{"processInformation": {"dataSetInformation": {"UUID": "00fe2655-02ad-4ded-925a-af9b8f1a27c8", "name": {"baseName": [{"value": "FASBA e.V. Baustroh 100 kg/m³", "lang": "de"}, {"value": "FASBA e.V. Baustroh 100 kg/m³ GaBi - 2024", "lang": "en"}], "functionalUnitFlowProperties": [{"value": "100 kg/m³", "lang": "en"}, {"value": "100 kg/m³", "lang": "de"}]}, "synonyms": [{"value": "Strohballen, Strohballendämmung, Strohdämmung", "lang": "de"}, {"value": "Straw bales, straw insulation, straw", "lang": "en"}], "classificationInformation": {"classification": [{"class": [{"value": "Dämmstoffe", "level": 0, "classId": "2"}, {"value": "Stroh", "level": 1, "classId": "2.23"}, {"value": "Strohballen", "level": 2, "classId": "2.23.01"}], "name": "OEKOBAU.DAT"}]}, "generalComment": [{"value": "Der vorliegende Bericht wurde im Auftrag des Fachverbands Strohballenbau Deutschland e. V. (FASBA) durchgeführt. Die Herstellung der Strohballen erfolgt durch die Baustroh GmbH in Verden vorwiegend aus Weizen- und Roggenstroh ohne Verwendung von zusätzlichen Einsatzstoffen. Die Rohdichte der Produkte liegt zwischen 85 und 115 kg/m³. Die hier publizierten Produktdaten sind repräsentativ für alle Baustrohballen des Fachverbands Baustrohballen Deutschland e.V. Zielmarkt der Produkte ist Deutschland.\r\nAls funktionale Einheit wurde 1 m³ Baustroh festgelegt.", "lang": "de"}, {"value": "This data set was developed on behalf of the Fachverband Strohballenbau Deutschland e. V. (FASBA) in the course of creating an EPD. The straw bales are produced by Baustroh GmbH in Verden, mainly from wheat and rye straw without the use of additional materials. Around 1000 m³ of building straw was produced in 2013. The bulk density of the products is between 85 and 115 kg/m³.", "lang": "en"}], "other": {"anies": [{"margins": 0.0, "description": [{"value": "keine", "lang": "de"}, {"value": "none", "lang": "en"}]}, {"scenario": [{"description": [{"value": "Szenario 1: 100% Verwertung (Verrottung)"}, {"value": "Szenario 1: 100% Energierückgewinnung", "lang": "de"}], "name": "Energierückgewinnung", "default": true}, {"description": [{"value": "Szenario 2: 90% Thermische Verwertung, 10% Deponierung von Materialverlusten"}, {"value": "Szenario 2: 100% Recycling", "lang": "de"}], "name": "Recycling", "default": false}]}, "<ns11:modules xmlns:ns11=\"http://openlca.org/epd_ilcd\" xmlns=\"http://lca.jrc.it/ILCD/Process\" xmlns:c=\"http://lca.jrc.it/ILCD/Contact\" xmlns:common=\"http://lca.jrc.it/ILCD/Common\" xmlns:epd=\"http://www.iai.kit.edu/EPD/2013\" xmlns:epd2=\"http://www.indata.network/EPD/2019\" xmlns:f=\"http://lca.jrc.it/ILCD/Flow\" xmlns:fp=\"http://lca.jrc.it/ILCD/FlowProperty\" xmlns:m=\"http://lca.jrc.it/ILCD/LCIAMethod\" xmlns:ns9=\"http://www.okworx.com/ILCD/Extensions/2018/Profile\" xmlns:s=\"http://lca.jrc.it/ILCD/Source\" xmlns:u=\"http://lca.jrc.it/ILCD/UnitGroup\" name=\"A1\"/>", "<ns11:modules xmlns:ns11=\"http://openlca.org/epd_ilcd\" xmlns=\"http://lca.jrc.it/ILCD/Process\" xmlns:c=\"http://lca.jrc.it/ILCD/Contact\" xmlns:common=\"http://lca.jrc.it/ILCD/Common\" xmlns:epd=\"http://www.iai.kit.edu/EPD/2013\" xmlns:epd2=\"http://www.indata.network/EPD/2019\" xmlns:f=\"http://lca.jrc.it/ILCD/Flow\" xmlns:fp=\"http://lca.jrc.it/ILCD/FlowProperty\" xmlns:m=\"http://lca.jrc.it/ILCD/LCIAMethod\" xmlns:ns9=\"http://www.okworx.com/ILCD/Extensions/2018/Profile\" xmlns:s=\"http://lca.jrc.it/ILCD/Source\" xmlns:u=\"http://lca.jrc.it/ILCD/UnitGroup\" name=\"A2\"/>", "<ns11:modules xmlns:ns11=\"http://openlca.org/epd_ilcd\" xmlns=\"http://lca.jrc.it/ILCD/Process\" xmlns:c=\"http://lca.jrc.it/ILCD/Contact\" xmlns:common=\"http://lca.jrc.it/ILCD/Common\" xmlns:epd=\"http://www.iai.kit.edu/EPD/2013\" xmlns:epd2=\"http://www.indata.network/EPD/2019\" xmlns:f=\"http://lca.jrc.it/ILCD/Flow\" xmlns:fp=\"http://lca.jrc.it/ILCD/FlowProperty\" xmlns:m=\"http://lca.jrc.it/ILCD/LCIAMethod\" xmlns:ns9=\"http://www.okworx.com/ILCD/Extensions/2018/Profile\" xmlns:s=\"http://lca.jrc.it/ILCD/Source\" xmlns:u=\"http://lca.jrc.it/ILCD/UnitGroup\" name=\"A3\"/>", "<ns11:modules xmlns:ns11=\"http://openlca.org/epd_ilcd\" xmlns=\"http://lca.jrc.it/ILCD/Process\" xmlns:c=\"http://lca.jrc.it/ILCD/Contact\" xmlns:common=\"http://lca.jrc.it/ILCD/Common\" xmlns:epd=\"http://www.iai.kit.edu/EPD/2013\" xmlns:epd2=\"http://www.indata.network/EPD/2019\" xmlns:f=\"http://lca.jrc.it/ILCD/Flow\" xmlns:fp=\"http://lca.jrc.it/ILCD/FlowProperty\" xmlns:m=\"http://lca.jrc.it/ILCD/LCIAMethod\" xmlns:ns9=\"http://www.okworx.com/ILCD/Extensions/2018/Profile\" xmlns:s=\"http://lca.jrc.it/ILCD/Source\" xmlns:u=\"http://lca.jrc.it/ILCD/UnitGroup\" name=\"A1-A3\"/>", "<ns11:modules xmlns:ns11=\"http://openlca.org/epd_ilcd\" xmlns=\"http://lca.jrc.it/ILCD/Process\" xmlns:c=\"http://lca.jrc.it/ILCD/Contact\" xmlns:common=\"http://lca.jrc.it/ILCD/Common\" xmlns:epd=\"http://www.iai.kit.edu/EPD/2013\" xmlns:epd2=\"http://www.indata.network/EPD/2019\" xmlns:f=\"http://lca.jrc.it/ILCD/Flow\" xmlns:fp=\"http://lca.jrc.it/ILCD/FlowProperty\" xmlns:m=\"http://lca.jrc.it/ILCD/LCIAMethod\" xmlns:ns9=\"http://www.okworx.com/ILCD/Extensions/2018/Profile\" xmlns:s=\"http://lca.jrc.it/ILCD/Source\" xmlns:u=\"http://lca.jrc.it/ILCD/UnitGroup\" name=\"A4\"/>", "<ns11:modules xmlns:ns11=\"http://openlca.org/epd_ilcd\" xmlns=\"http://lca.jrc.it/ILCD/Process\" xmlns:c=\"http://lca.jrc.it/ILCD/Contact\" xmlns:common=\"http://lca.jrc.it/ILCD/Common\" xmlns:epd=\"http://www.iai.kit.edu/EPD/2013\" xmlns:epd2=\"http://www.indata.network/EPD/2019\" xmlns:f=\"http://lca.jrc.it/ILCD/Flow\" xmlns:fp=\"http://lca.jrc.it/ILCD/FlowProperty\" xmlns:m=\"http://lca.jrc.it/ILCD/LCIAMethod\" xmlns:ns9=\"http://www.okworx.com/ILCD/Extensions/2018/Profile\" xmlns:s=\"http://lca.jrc.it/ILCD/Source\" xmlns:u=\"http://lca.jrc.it/ILCD/UnitGroup\" name=\"A5\"/>", "<ns11:modules xmlns:ns11=\"http://openlca.org/epd_ilcd\" xmlns=\"http://lca.jrc.it/ILCD/Process\" xmlns:c=\"http://lca.jrc.it/ILCD/Contact\" xmlns:common=\"http://lca.jrc.it/ILCD/Common\" xmlns:epd=\"http://www.iai.kit.edu/EPD/2013\" xmlns:epd2=\"http://www.indata.network/EPD/2019\" xmlns:f=\"http://lca.jrc.it/ILCD/Flow\" xmlns:fp=\"http://lca.jrc.it/ILCD/FlowProperty\" xmlns:m=\"http://lca.jrc.it/ILCD/LCIAMethod\" xmlns:ns9=\"http://www.okworx.com/ILCD/Extensions/2018/Profile\" xmlns:s=\"http://lca.jrc.it/ILCD/Source\" xmlns:u=\"http://lca.jrc.it/ILCD/UnitGroup\" name=\"B1\"/>", "<ns11:modules xmlns:ns11=\"http://openlca.org/epd_ilcd\" xmlns=\"http://lca.jrc.it/ILCD/Process\" xmlns:c=\"http://lca.jrc.it/ILCD/Contact\" xmlns:common=\"http://lca.jrc.it/ILCD/Common\" xmlns:epd=\"http://www.iai.kit.edu/EPD/2013\" xmlns:epd2=\"http://www.indata.network/EPD/2019\" xmlns:f=\"http://lca.jrc.it/ILCD/Flow\" xmlns:fp=\"http://lca.jrc.it/ILCD/FlowProperty\" xmlns:m=\"http://lca.jrc.it/ILCD/LCIAMethod\" xmlns:ns9=\"http://www.okworx.com/ILCD/Extensions/2018/Profile\" xmlns:s=\"http://lca.jrc.it/ILCD/Source\" xmlns:u=\"http://lca.jrc.it/ILCD/UnitGroup\" name=\"B2\"/>", "<ns11:modules xmlns:ns11=\"http://openlca.org/epd_ilcd\" xmlns=\"http://lca.jrc.it/ILCD/Process\" xmlns:c=\"http://lca.jrc.it/ILCD/Contact\" xmlns:common=\"http://lca.jrc.it/ILCD/Common\" xmlns:epd=\"http://www.iai.kit.edu/EPD/2013\" xmlns:epd2=\"http://www.indata.network/EPD/2019\" xmlns:f=\"http://lca.jrc.it/ILCD/Flow\" xmlns:fp=\"http://lca.jrc.it/ILCD/FlowProperty\" xmlns:m=\"http://lca.jrc.it/ILCD/LCIAMethod\" xmlns:ns9=\"http://www.okworx.com/ILCD/Extensions/2018/Profile\" xmlns:s=\"http://lca.jrc.it/ILCD/Source\" xmlns:u=\"http://lca.jrc.it/ILCD/UnitGroup\" name=\"B3\"/>", "<ns11:modules xmlns:ns11=\"http://openlca.org/epd_ilcd\" xmlns=\"http://lca.jrc.it/ILCD/Process\" xmlns:c=\"http://lca.jrc.it/ILCD/Contact\" xmlns:common=\"http://lca.jrc.it/ILCD/Common\" xmlns:epd=\"http://www.iai.kit.edu/EPD/2013\" xmlns:epd2=\"http://www.indata.network/EPD/2019\" xmlns:f=\"http://lca.jrc.it/ILCD/Flow\" xmlns:fp=\"http://lca.jrc.it/ILCD/FlowProperty\" xmlns:m=\"http://lca.jrc.it/ILCD/LCIAMethod\" xmlns:ns9=\"http://www.okworx.com/ILCD/Extensions/2018/Profile\" xmlns:s=\"http://lca.jrc.it/ILCD/Source\" xmlns:u=\"http://lca.jrc.it/ILCD/UnitGroup\" name=\"B4\"/>", "<ns11:modules xmlns:ns11=\"http://openlca.org/epd_ilcd\" xmlns=\"http://lca.jrc.it/ILCD/Process\" xmlns:c=\"http://lca.jrc.it/ILCD/Contact\" xmlns:common=\"http://lca.jrc.it/ILCD/Common\" xmlns:epd=\"http://www.iai.kit.edu/EPD/2013\" xmlns:epd2=\"http://www.indata.network/EPD/2019\" xmlns:f=\"http://lca.jrc.it/ILCD/Flow\" xmlns:fp=\"http://lca.jrc.it/ILCD/FlowProperty\" xmlns:m=\"http://lca.jrc.it/ILCD/LCIAMethod\" xmlns:ns9=\"http://www.okworx.com/ILCD/Extensions/2018/Profile\" xmlns:s=\"http://lca.jrc.it/ILCD/Source\" xmlns:u=\"http://lca.jrc.it/ILCD/UnitGroup\" name=\"B5\"/>", "<ns11:modules xmlns:ns11=\"http://openlca.org/epd_ilcd\" xmlns=\"http://lca.jrc.it/ILCD/Process\" xmlns:c=\"http://lca.jrc.it/ILCD/Contact\" xmlns:common=\"http://lca.jrc.it/ILCD/Common\" xmlns:epd=\"http://www.iai.kit.edu/EPD/2013\" xmlns:epd2=\"http://www.indata.network/EPD/2019\" xmlns:f=\"http://lca.jrc.it/ILCD/Flow\" xmlns:fp=\"http://lca.jrc.it/ILCD/FlowProperty\" xmlns:m=\"http://lca.jrc.it/ILCD/LCIAMethod\" xmlns:ns9=\"http://www.okworx.com/ILCD/Extensions/2018/Profile\" xmlns:s=\"http://lca.jrc.it/ILCD/Source\" xmlns:u=\"http://lca.jrc.it/ILCD/UnitGroup\" name=\"B6\"/>", "<ns11:modules xmlns:ns11=\"http://openlca.org/epd_ilcd\" xmlns=\"http://lca.jrc.it/ILCD/Process\" xmlns:c=\"http://lca.jrc.it/ILCD/Contact\" xmlns:common=\"http://lca.jrc.it/ILCD/Common\" xmlns:epd=\"http://www.iai.kit.edu/EPD/2013\" xmlns:epd2=\"http://www.indata.network/EPD/2019\" xmlns:f=\"http://lca.jrc.it/ILCD/Flow\" xmlns:fp=\"http://lca.jrc.it/ILCD/FlowProperty\" xmlns:m=\"http://lca.jrc.it/ILCD/LCIAMethod\" xmlns:ns9=\"http://www.okworx.com/ILCD/Extensions/2018/Profile\" xmlns:s=\"http://lca.jrc.it/ILCD/Source\" xmlns:u=\"http://lca.jrc.it/ILCD/UnitGroup\" name=\"B7\"/>", "<ns11:modules xmlns:ns11=\"http://openlca.org/epd_ilcd\" xmlns=\"http://lca.jrc.it/ILCD/Process\" xmlns:c=\"http://lca.jrc.it/ILCD/Contact\" xmlns:common=\"http://lca.jrc.it/ILCD/Common\" xmlns:epd=\"http://www.iai.kit.edu/EPD/2013\" xmlns:epd2=\"http://www.indata.network/EPD/2019\" xmlns:f=\"http://lca.jrc.it/ILCD/Flow\" xmlns:fp=\"http://lca.jrc.it/ILCD/FlowProperty\" xmlns:m=\"http://lca.jrc.it/ILCD/LCIAMethod\" xmlns:ns9=\"http://www.okworx.com/ILCD/Extensions/2018/Profile\" xmlns:s=\"http://lca.jrc.it/ILCD/Source\" xmlns:u=\"http://lca.jrc.it/ILCD/UnitGroup\" name=\"C1\" scenario=\"Energierückgewinnung\"/>", "<ns11:modules xmlns:ns11=\"http://openlca.org/epd_ilcd\" xmlns=\"http://lca.jrc.it/ILCD/Process\" xmlns:c=\"http://lca.jrc.it/ILCD/Contact\" xmlns:common=\"http://lca.jrc.it/ILCD/Common\" xmlns:epd=\"http://www.iai.kit.edu/EPD/2013\" xmlns:epd2=\"http://www.indata.network/EPD/2019\" xmlns:f=\"http://lca.jrc.it/ILCD/Flow\" xmlns:fp=\"http://lca.jrc.it/ILCD/FlowProperty\" xmlns:m=\"http://lca.jrc.it/ILCD/LCIAMethod\" xmlns:ns9=\"http://www.okworx.com/ILCD/Extensions/2018/Profile\" xmlns:s=\"http://lca.jrc.it/ILCD/Source\" xmlns:u=\"http://lca.jrc.it/ILCD/UnitGroup\" name=\"C2\" scenario=\"Energierückgewinnung\"/>", "<ns11:modules xmlns:ns11=\"http://openlca.org/epd_ilcd\" xmlns=\"http://lca.jrc.it/ILCD/Process\" xmlns:c=\"http://lca.jrc.it/ILCD/Contact\" xmlns:common=\"http://lca.jrc.it/ILCD/Common\" xmlns:epd=\"http://www.iai.kit.edu/EPD/2013\" xmlns:epd2=\"http://www.indata.network/EPD/2019\" xmlns:f=\"http://lca.jrc.it/ILCD/Flow\" xmlns:fp=\"http://lca.jrc.it/ILCD/FlowProperty\" xmlns:m=\"http://lca.jrc.it/ILCD/LCIAMethod\" xmlns:ns9=\"http://www.okworx.com/ILCD/Extensions/2018/Profile\" xmlns:s=\"http://lca.jrc.it/ILCD/Source\" xmlns:u=\"http://lca.jrc.it/ILCD/UnitGroup\" name=\"C3\" scenario=\"Energierückgewinnung\"/>", "<ns11:modules xmlns:ns11=\"http://openlca.org/epd_ilcd\" xmlns=\"http://lca.jrc.it/ILCD/Process\" xmlns:c=\"http://lca.jrc.it/ILCD/Contact\" xmlns:common=\"http://lca.jrc.it/ILCD/Common\" xmlns:epd=\"http://www.iai.kit.edu/EPD/2013\" xmlns:epd2=\"http://www.indata.network/EPD/2019\" xmlns:f=\"http://lca.jrc.it/ILCD/Flow\" xmlns:fp=\"http://lca.jrc.it/ILCD/FlowProperty\" xmlns:m=\"http://lca.jrc.it/ILCD/LCIAMethod\" xmlns:ns9=\"http://www.okworx.com/ILCD/Extensions/2018/Profile\" xmlns:s=\"http://lca.jrc.it/ILCD/Source\" xmlns:u=\"http://lca.jrc.it/ILCD/UnitGroup\" name=\"C4\" scenario=\"Energierückgewinnung\"/>", "<ns11:modules xmlns:ns11=\"http://openlca.org/epd_ilcd\" xmlns=\"http://lca.jrc.it/ILCD/Process\" xmlns:c=\"http://lca.jrc.it/ILCD/Contact\" xmlns:common=\"http://lca.jrc.it/ILCD/Common\" xmlns:epd=\"http://www.iai.kit.edu/EPD/2013\" xmlns:epd2=\"http://www.indata.network/EPD/2019\" xmlns:f=\"http://lca.jrc.it/ILCD/Flow\" xmlns:fp=\"http://lca.jrc.it/ILCD/FlowProperty\" xmlns:m=\"http://lca.jrc.it/ILCD/LCIAMethod\" xmlns:ns9=\"http://www.okworx.com/ILCD/Extensions/2018/Profile\" xmlns:s=\"http://lca.jrc.it/ILCD/Source\" xmlns:u=\"http://lca.jrc.it/ILCD/UnitGroup\" name=\"D\" scenario=\"Energierückgewinnung\"/>", "<ns11:modules xmlns:ns11=\"http://openlca.org/epd_ilcd\" xmlns=\"http://lca.jrc.it/ILCD/Process\" xmlns:c=\"http://lca.jrc.it/ILCD/Contact\" xmlns:common=\"http://lca.jrc.it/ILCD/Common\" xmlns:epd=\"http://www.iai.kit.edu/EPD/2013\" xmlns:epd2=\"http://www.indata.network/EPD/2019\" xmlns:f=\"http://lca.jrc.it/ILCD/Flow\" xmlns:fp=\"http://lca.jrc.it/ILCD/FlowProperty\" xmlns:m=\"http://lca.jrc.it/ILCD/LCIAMethod\" xmlns:ns9=\"http://www.okworx.com/ILCD/Extensions/2018/Profile\" xmlns:s=\"http://lca.jrc.it/ILCD/Source\" xmlns:u=\"http://lca.jrc.it/ILCD/UnitGroup\" name=\"C1\" scenario=\"Recycling\"/>", "<ns11:modules xmlns:ns11=\"http://openlca.org/epd_ilcd\" xmlns=\"http://lca.jrc.it/ILCD/Process\" xmlns:c=\"http://lca.jrc.it/ILCD/Contact\" xmlns:common=\"http://lca.jrc.it/ILCD/Common\" xmlns:epd=\"http://www.iai.kit.edu/EPD/2013\" xmlns:epd2=\"http://www.indata.network/EPD/2019\" xmlns:f=\"http://lca.jrc.it/ILCD/Flow\" xmlns:fp=\"http://lca.jrc.it/ILCD/FlowProperty\" xmlns:m=\"http://lca.jrc.it/ILCD/LCIAMethod\" xmlns:ns9=\"http://www.okworx.com/ILCD/Extensions/2018/Profile\" xmlns:s=\"http://lca.jrc.it/ILCD/Source\" xmlns:u=\"http://lca.jrc.it/ILCD/UnitGroup\" name=\"C2\" scenario=\"Recycling\"/>", "<ns11:modules xmlns:ns11=\"http://openlca.org/epd_ilcd\" xmlns=\"http://lca.jrc.it/ILCD/Process\" xmlns:c=\"http://lca.jrc.it/ILCD/Contact\" xmlns:common=\"http://lca.jrc.it/ILCD/Common\" xmlns:epd=\"http://www.iai.kit.edu/EPD/2013\" xmlns:epd2=\"http://www.indata.network/EPD/2019\" xmlns:f=\"http://lca.jrc.it/ILCD/Flow\" xmlns:fp=\"http://lca.jrc.it/ILCD/FlowProperty\" xmlns:m=\"http://lca.jrc.it/ILCD/LCIAMethod\" xmlns:ns9=\"http://www.okworx.com/ILCD/Extensions/2018/Profile\" xmlns:s=\"http://lca.jrc.it/ILCD/Source\" xmlns:u=\"http://lca.jrc.it/ILCD/UnitGroup\" name=\"C3\" scenario=\"Recycling\"/>", "<ns11:modules xmlns:ns11=\"http://openlca.org/epd_ilcd\" xmlns=\"http://lca.jrc.it/ILCD/Process\" xmlns:c=\"http://lca.jrc.it/ILCD/Contact\" xmlns:common=\"http://lca.jrc.it/ILCD/Common\" xmlns:epd=\"http://www.iai.kit.edu/EPD/2013\" xmlns:epd2=\"http://www.indata.network/EPD/2019\" xmlns:f=\"http://lca.jrc.it/ILCD/Flow\" xmlns:fp=\"http://lca.jrc.it/ILCD/FlowProperty\" xmlns:m=\"http://lca.jrc.it/ILCD/LCIAMethod\" xmlns:ns9=\"http://www.okworx.com/ILCD/Extensions/2018/Profile\" xmlns:s=\"http://lca.jrc.it/ILCD/Source\" xmlns:u=\"http://lca.jrc.it/ILCD/UnitGroup\" name=\"C4\" scenario=\"Recycling\"/>", "<ns11:modules xmlns:ns11=\"http://openlca.org/epd_ilcd\" xmlns=\"http://lca.jrc.it/ILCD/Process\" xmlns:c=\"http://lca.jrc.it/ILCD/Contact\" xmlns:common=\"http://lca.jrc.it/ILCD/Common\" xmlns:epd=\"http://www.iai.kit.edu/EPD/2013\" xmlns:epd2=\"http://www.indata.network/EPD/2019\" xmlns:f=\"http://lca.jrc.it/ILCD/Flow\" xmlns:fp=\"http://lca.jrc.it/ILCD/FlowProperty\" xmlns:m=\"http://lca.jrc.it/ILCD/LCIAMethod\" xmlns:ns9=\"http://www.okworx.com/ILCD/Extensions/2018/Profile\" xmlns:s=\"http://lca.jrc.it/ILCD/Source\" xmlns:u=\"http://lca.jrc.it/ILCD/UnitGroup\" name=\"D\" scenario=\"Recycling\"/>"]}}, "quantitativeReference": {"referenceToReferenceFlow": [0], "type": "Reference flow(s)"}, "time": {"referenceYear": 2024, "dataSetValidUntil": 2029, "timeRepresentativenessDescription": [{"value": "Die Strohsorten im Produkt, die Transportdistanz zur Baustelle und die Beladung des LKW wurden vom Fachverband für Strohballenbau übermittelt und beziehen sich auf das Jahr 2022. ", "lang": "de"}, {"value": "The straw types in the product, the transport distance to the construction site and the lorry load were provided by the straw bale construction association and refer to the year 2022. ", "lang": "en"}], "other": {"anies": [{"name": "publicationDateOfEPD", "value": 1734912000000}]}}, "geography": {"locationOfOperationSupplyOrProduction": {"descriptionOfRestrictions": [{"value": "Durchschnittliche Transportdistanz vom Werk zu den Baustellen wurde mit 100 km innerhalb Deutschlands angenommen.", "lang": "de"}, {"value": "The average transport distance from the factory to the construction sites was assumed to be 100 km within Germany.", "lang": "en"}], "location": "DE"}}, "technology": {"technologyDescriptionAndIncludedProcesses": [{"value": "Herstellungsprozess: Die Herstellung der Strohballen inkludiert sämtliche landwirtschaftliche Prozesse von der Bodenbearbeitung und der Aussaat des Korns über die Kultivierung der Pflanzen bis hin zur Ernte des Getreides. Nach der Ernte wird das Stroh auf dem Acker ohne Verwendung von zusätzlichen Einsatzstoffen zu Ballen gepresst und mit Polypropylenschnüren verschnürt.\r\n\r\nDie Rohdichte der Produkte liegt zwischen 85 und 115 kg/m³. Baustroh ist in Ballenform in den Abmessungen H x B x L 200-700 mm x 300 bis 900 mm x 500 bis 3000 mm erhältlich. Die Ballen werden mit Polypropylen-Schnüren gebunden.\r\nWärmeleitfähigkeit λ 10,tr= 0,044 W/(mK)\r\nBemessungswert der Wärmeleitfähigkeit quer zur Halmrichtung  λ=0,052 W/(mK)", "lang": "de"}, {"value": "Production process: The production of straw bales includes all agricultural processes from soil cultivation and sowing the grain to cultivating the plants and harvesting the grain. After harvesting, the straw is pressed into bales in the field without the use of additional materials and tied with polypropylene twine.\n\nThe bulk density of the products is between 85 and 115 kg/m³. Building straw is available in bale form in the dimensions H x W x L 200-700 mm x 300 to 900 mm x 500 to 3000 mm. The bales are bound with polypropylene cords.\nThermal conductivity λ 10,tr= 0.044 W/(mK)\nRated value of thermal conductivity transverse to the direction of the stalk λ=0.052 W/(mK)", "lang": "en"}], "technologicalApplicability": [{"value": "Die Strohballen des FASBA e.V. werden als dämmende Ausfachung in einer Holzkonstruktion eingesetzt. ", "lang": "de"}, {"value": "The straw bales from FASBA e.V. are used as insulating infill in a timber construction. ", "lang": "en"}], "referenceToTechnologyPictogramme": {"shortDescription": [{"value": "Fasba Titelblatt", "lang": "en"}], "type": "source data set", "refObjectId": "449e5220-565d-4e27-973f-1bb783023802", "version": "00.00.001", "uri": "http://openlca.org/ilcd/resource/sources/449e5220-565d-4e27-973f-1bb783023802"}, "referenceToTechnologyFlowDiagrammOrPicture": [{"shortDescription": [{"value": "Fasba Strohballen LifeCycle Flussdiagramm", "lang": "en"}], "type": "source data set", "refObjectId": "3f7d422e-df93-46f1-b4be-75db38013f54", "version": "00.00.001", "uri": "http://openlca.org/ilcd/resource/sources/3f7d422e-df93-46f1-b4be-75db38013f54"}]}}, "modellingAndValidation": {"LCIMethodAndAllocation": {"typeOfDataSet": "EPD", "referenceToLCAMethodDetails": [{"shortDescription": [{"value": "PKR Bau EPD GmbH PKR-Code: 2.22.5 Version 12.0 Stand 20.09.2023 \"Dämmstoffe aus nachwachsenden Rohstoffen\"", "lang": "de"}], "type": "source data set", "refObjectId": "7d5585c9-0fd2-4b95-bf48-722f260e46b0", "version": "00.00.000"}], "other": {"anies": [{"name": "subType", "value": "specific dataset"}]}}, "dataSourcesTreatmentAndRepresentativeness": {"referenceToDataSource": [{"shortDescription": [{"value": "GaBi database (general)", "lang": "en"}], "type": "source data set", "refObjectId": "28d74cc0-db8b-4d7e-bc44-5f6d56ce0c4a", "version": "00.03.002"}, {"shortDescription": [{"value": "Sphera MLC (fka GaBi) Databases Edition 2024", "lang": "en"}], "type": "source data set", "refObjectId": "7443b962-0446-4d69-8aa7-8055a6b1614a", "version": "00.01.000"}, {"shortDescription": [{"value": "Software: LCA for Experts (Version 10.9.0.20)", "lang": "de"}], "type": "source data set", "refObjectId": "7fd0f1bc-66d5-45fa-8f81-b96451d3ca7c", "version": "00.00.002"}], "useAdviceForDataSet": [{"value": "Anmerkung zur Vergleichbarkeit: Ein Vergleich mit anderen Produkten ist nur mit einer vergleichbaren Anwendung im Gebäude sinnvoll. Grundsätzlich ist eine Gegenüberstellung oder die Bewertung von EPD Daten nur möglich, wenn alle zu vergleichenden Datensätze nach EN 15804 erstellt wurden und die produktspezifischen Leistungsmerkmale berücksichtigt werden.", "lang": "de"}, {"value": "Note on comparability: A comparison with other products is only meaningful with a comparable application in the building. In principle, a comparison or evaluation of EPD data is only possible if all data sets to be compared were created in accordance with EN 15804 and the product-specific performance characteristics are taken into account.", "lang": "en"}], "other": {"anies": [{"name": "referenceToOriginalEPD", "value": {"shortDescription": {"value": "Bau EPD GmbH EPD GABI FASBA 2024-1", "defaultValue": "Bau EPD GmbH EPD GABI FASBA 2024-1", "lstrings": [{"lang": "de", "value": "Bau EPD GmbH EPD GABI FASBA 2024-1"}]}, "version": {"version": 1, "majorVersion": 0, "minorVersion": 0, "subMinorVersion": 1, "zero": false, "versionString": "00.00.001"}, "uri": "http://openlca.org/ilcd/resource/sources/ed07cc37-ac91-43e7-9629-c0e795e338c5", "href": "http://openlca.org/ilcd/resource/sources/ed07cc37-ac91-43e7-9629-c0e795e338c5", "type": "source data set", "uuid": {"uuid": "d06312e6-2c2d-442d-ab40-f73fe7ef7166"}, "refObjectId": "d06312e6-2c2d-442d-ab40-f73fe7ef7166", "versionAsString": "00.00.001", "resourceURLs": ["https://oekobaudat.de/OEKOBAU.DAT/resource/sources/d06312e6-2c2d-442d-ab40-f73fe7ef7166/BAU-EPD-Fasba-2024-1-GaBi-Baustroh-20241223-Webseite.pdf?version=00.00.001"]}}]}}, "validation": {"review": [{"reviewDetails": [{"value": "none", "lang": "en"}, {"value": "keine", "lang": "de"}], "referenceToNameOfReviewerAndInstitution": [{"shortDescription": [{"value": "Bau EPD GmbH", "lang": "de"}, {"value": "Bau EPD GmbH", "lang": "en"}], "type": "contact data set", "refObjectId": "42398bec-0af8-444e-9221-d40be4c4f553", "version": "00.00.007", "uri": "http://openlca.org/ilcd/resource/contacts/42398bec-0af8-444e-9221-d40be4c4f553"}, {"shortDescription": [{"value": "Verifier Gschösser, Florian", "lang": "de"}], "type": "contact data set", "refObjectId": "da875289-3cae-4746-91a3-e7b476932b81", "version": "00.00.005"}, {"shortDescription": [{"value": "Verifier Schindler, Angela", "lang": "de"}], "type": "contact data set", "refObjectId": "495354d6-9c79-4c06-8313-0b4655316693", "version": "00.00.003"}], "type": "Accredited third party review"}]}, "complianceDeclarations": {"compliance": [{"referenceToComplianceSystem": {"shortDescription": [{"value": "ISO 14025", "lang": "en"}], "type": "source data set", "refObjectId": "4f2eb655-6e44-4874-a95a-e28f5442cd4d", "version": "00.00.001"}}, {"referenceToComplianceSystem": {"shortDescription": [{"value": "EN 15804+A2 (EF 3.1)", "lang": "de"}, {"value": "EN 15804+A2 (EF 3.1)", "lang": "en"}], "type": "source data set", "refObjectId": "d4aa3ec7-b1d7-4a4a-a6cb-37af88dcc902", "version": "00.01.000"}}]}}, "administrativeInformation": {"dataGenerator": {"referenceToPersonOrEntityGeneratingTheDataSet": [{"shortDescription": [{"value": "IBO Institut für Baubiologie und Bauökologie", "lang": "de"}], "type": "contact data set", "refObjectId": "50fccae1-aef9-4e76-acf5-fe0428976e43", "version": "00.00.003"}]}, "dataEntryBy": {"timeStamp": 1742455037279, "referenceToDataSetFormat": [{"shortDescription": [{"value": "ILCD format", "lang": "en"}], "type": "source data set", "refObjectId": "a97a0155-0234-4b87-b4ce-a45da52f2a40", "version": "01.00.000", "uri": "http://lca.jrc.ec.europa.eu/lcainfohub/sample_data/ilcd/sources/ILCD_Format_a97a0155-0234-4b87-b4ce-a45da52f2a40_01.00.000.xml"}, {"shortDescription": [{"value": "EPD Data Format Extensions v1.2", "lang": "en"}, {"value": "EPD-Datenformaterweiterungen v1.2", "lang": "de"}], "type": "source data set", "refObjectId": "a29449fd-aa2f-4de8-b5d7-4b06b43c6fde", "version": "00.01.000"}], "referenceToPersonOrEntityEnteringTheData": {"shortDescription": [{"value": "Bau EPD GmbH", "lang": "de"}, {"value": "Bau EPD GmbH", "lang": "en"}], "type": "contact data set", "refObjectId": "42398bec-0af8-444e-9221-d40be4c4f553", "version": "00.00.007", "uri": "http://openlca.org/ilcd/resource/contacts/42398bec-0af8-444e-9221-d40be4c4f553"}}, "publicationAndOwnership": {"dataSetVersion": "00.00.016", "referenceToPrecedingDataSetVersion": [{"shortDescription": [{"value": "FASBA e.V. Baustroh", "lang": "de"}, {"value": "FASBA e.V. Baustroh 100 kg/m³ GaBi - 2019", "lang": "en"}], "otherAttributes": {"{http://greendelta.com/epd-editor}referenceYear": "2019", "{http://greendelta.com/epd-editor}database": "GaBi"}, "type": "process data set", "refObjectId": "d2d1b29f-8dd7-4373-ab2a-de57acd51e72", "version": "00.00.044"}], "referenceToRegistrationAuthority": {"shortDescription": [{"value": "Bau EPD GmbH", "lang": "de"}, {"value": "Bau EPD GmbH", "lang": "en"}], "type": "contact data set", "refObjectId": "42398bec-0af8-444e-9221-d40be4c4f553", "version": "00.00.007", "uri": "http://openlca.org/ilcd/resource/contacts/42398bec-0af8-444e-9221-d40be4c4f553"}, "registrationNumber": "BAU-EPD-2024-1-GaBi-Baustroh", "referenceToOwnershipOfDataSet": {"shortDescription": [{"value": "FASBA e.V.", "lang": "en"}], "type": "contact data set", "refObjectId": "9828b42f-275d-4651-9853-7abe6183f6b6", "version": "00.00.002", "uri": "http://openlca.org/ilcd/resource/contacts/9828b42f-275d-4651-9853-7abe6183f6b6"}, "copyright": true, "licenseType": "Free of charge for all users and uses", "accessRestrictions": [{"value": "keine", "lang": "de"}, {"value": "none", "lang": "en"}], "other": {"anies": [{"name": "referenceToPublisher", "value": {"shortDescription": [{"value": "Bau EPD GmbH", "lang": "de"}, {"value": "Bau EPD GmbH", "lang": "en"}], "type": "contact data set", "refObjectId": "42398bec-0af8-444e-9221-d40be4c4f553", "version": "00.00.007", "uri": "http://openlca.org/ilcd/resource/contacts/42398bec-0af8-444e-9221-d40be4c4f553"}}]}}}, "exchanges": {"exchange": [{"dataSetInternalID": 0, "referenceToFlowDataSet": {"shortDescription": [{"value": "Strohballen", "lang": "de"}], "type": "flow data set", "refObjectId": "7acdb69c-7d9b-400a-bbeb-74c352c006d3", "version": "00.00.011", "uri": "http://openlca.org/ilcd/resource/flows/7acdb69c-7d9b-400a-bbeb-74c352c006d3"}, "meanAmount": 1.0, "resultingAmount": 1.0, "referenceFlow": true, "resultingflowAmount": 1.0, "flowProperties": [{"name": [{"lang": "en", "value": "Volume"}, {"lang": "de", "value": "Volumen"}], "uuid": "93a60a56-a3c8-22da-a746-0800200c9a66", "referenceFlowProperty": true, "meanValue": 1.0, "referenceUnit": "m3", "unitGroupUUID": "cd950537-0a98-4044-9ba7-9f9a68d0a504"}, {"name": [{"lang": "de", "value": "Masse"}, {"lang": "en", "value": "Mass"}], "uuid": "93a60a56-a3c8-11da-a746-0800200b9a66", "meanValue": 100.0}], "materialProperties": [{"name": "gross density", "value": "100.0", "unit": "kg/m^3", "unitDescription": "kilograms per cubic metre"}], "typeOfFlow": "Product flow", "classification": {"classHierarchy": "Dämmstoffe / Strohdämmung", "name": "ilcd"}}, {"dataSetInternalID": 1, "referenceToFlowDataSet": {"shortDescription": [{"value": "Use of renewable primary energy (PERE)", "lang": "en"}, {"value": "Erneuerbare Primärenergie als Energieträger (PERE)", "lang": "de"}, {"value": "Uso de energía primaria renovable excluyendo los recursos de energía primaria renovable utilizada como materia prima (PERE)", "lang": "es"}], "type": "flow data set", "refObjectId": "20f32be5-0398-4288-9b6d-accddd195317", "version": "38.00.000", "uri": "../flows/20f32be5-0398-4288-9b6d-accddd195317.xml"}, "exchange direction": "INPUT", "meanAmount": 0.0, "other": {"anies": [{"value": "291.32897428468004", "module": "A1-A3"}, {"value": "2.98444096065488", "module": "A4"}, {"value": "90.9146848663361", "module": "A5"}, {"value": "0.0", "module": "B1"}, {"value": "0.0", "module": "B2"}, {"value": "0.0", "module": "B3"}, {"value": "0.0", "module": "B4"}, {"value": "0.0", "module": "B5"}, {"value": "0.0", "module": "B6"}, {"value": "0.0", "module": "B7"}, {"value": "0.0", "module": "C1", "scenario": "Energierückgewinnung"}, {"value": "1.43435960677528", "module": "C2", "scenario": "Energierückgewinnung"}, {"value": "1522.2833155023307", "module": "C3", "scenario": "Energierückgewinnung"}, {"value": "0.0", "module": "C4", "scenario": "Energierückgewinnung"}, {"value": "-334.4141388318348", "module": "D", "scenario": "Energierückgewinnung"}, {"value": "0.0", "module": "C1", "scenario": "Recycling"}, {"value": "1.43435960677528", "module": "C2", "scenario": "Recycling"}, {"value": "1556.85647501767", "module": "C3", "scenario": "Recycling"}, {"value": "0.0", "module": "C4", "scenario": "Recycling"}, {"value": "-17.490123997693914", "module": "D", "scenario": "Recycling"}, {"name": "referenceToUnitGroupDataSet", "value": {"shortDescription": [{"value": "MJ", "lang": "en"}], "type": "unit group data set", "refObjectId": "93a60a57-a3c8-11da-a746-0800200c9a66", "version": "03.00.000", "uri": "../unitgroups/93a60a57-a3c8-11da-a746-0800200c9a66.xml"}}]}, "flowProperties": [], "typeOfFlow": "Other flow", "classification": {"classHierarchy": "Quantities", "name": "GaBiCategories"}}, {"dataSetInternalID": 2, "referenceToFlowDataSet": {"shortDescription": [{"value": "Use of renewable primary energy resources used as raw materials (PERM)", "lang": "en"}, {"value": "Erneuerbare Primärenergie zur stofflichen Nutzung (PERM)", "lang": "de"}, {"value": "Uso de energía primaria renovable utilizada como materia prima (PERM)", "lang": "es"}], "type": "flow data set", "refObjectId": "fb3ec0de-548d-4508-aea5-00b73bf6f702", "version": "38.00.000", "uri": "../flows/fb3ec0de-548d-4508-aea5-00b73bf6f702.xml"}, "exchange direction": "INPUT", "meanAmount": 0.0, "other": {"anies": [{"value": "1510.0", "module": "A1-A3"}, {"value": "0.0", "module": "A4"}, {"value": "0.0", "module": "A5"}, {"value": "0.0", "module": "B1"}, {"value": "0.0", "module": "B2"}, {"value": "0.0", "module": "B3"}, {"value": "0.0", "module": "B4"}, {"value": "0.0", "module": "B5"}, {"value": "0.0", "module": "B6"}, {"value": "0.0", "module": "B7"}, {"value": "0.0", "module": "C1", "scenario": "Energierückgewinnung"}, {"value": "0.0", "module": "C2", "scenario": "Energierückgewinnung"}, {"value": "-1510.0", "module": "C3", "scenario": "Energierückgewinnung"}, {"value": "0.0", "module": "C4", "scenario": "Energierückgewinnung"}, {"value": "0.0", "module": "D", "scenario": "Energierückgewinnung"}, {"value": "0.0", "module": "C1", "scenario": "Recycling"}, {"value": "0.0", "module": "C2", "scenario": "Recycling"}, {"value": "-1510.0", "module": "C3", "scenario": "Recycling"}, {"value": "0.0", "module": "C4", "scenario": "Recycling"}, {"value": "0.0", "module": "D", "scenario": "Recycling"}, {"name": "referenceToUnitGroupDataSet", "value": {"shortDescription": [{"value": "MJ", "lang": "en"}], "type": "unit group data set", "refObjectId": "93a60a57-a3c8-11da-a746-0800200c9a66", "version": "03.00.000", "uri": "../unitgroups/93a60a57-a3c8-11da-a746-0800200c9a66.xml"}}]}, "flowProperties": [], "typeOfFlow": "Other flow", "classification": {"classHierarchy": "Quantities", "name": "GaBiCategories"}}, {"dataSetInternalID": 3, "referenceToFlowDataSet": {"shortDescription": [{"value": "Total use of renewable primary energy resources (PERT)", "lang": "en"}, {"value": "Total erneuerbare Primärenergie (PERT)", "lang": "de"}, {"value": "Uso total de la energía primaria renovable (energía primaria y recursos de energía primaria renovable utilizada como materia prima) (PERT)", "lang": "es"}], "type": "flow data set", "refObjectId": "53f97275-fa8a-4cdd-9024-65936002acd0", "version": "30.00.000", "uri": "../flows/53f97275-fa8a-4cdd-9024-65936002acd0.xml"}, "exchange direction": "INPUT", "meanAmount": 0.0, "other": {"anies": [{"value": "1801.32897428468", "module": "A1-A3"}, {"value": "2.98444096065488", "module": "A4"}, {"value": "90.9146848663361", "module": "A5"}, {"value": "0.0", "module": "B1"}, {"value": "0.0", "module": "B2"}, {"value": "0.0", "module": "B3"}, {"value": "0.0", "module": "B4"}, {"value": "0.0", "module": "B5"}, {"value": "0.0", "module": "B6"}, {"value": "0.0", "module": "B7"}, {"value": "0.0", "module": "C1", "scenario": "Energierückgewinnung"}, {"value": "1.43435960677528", "module": "C2", "scenario": "Energierückgewinnung"}, {"value": "12.283315502330652", "module": "C3", "scenario": "Energierückgewinnung"}, {"value": "0.0", "module": "C4", "scenario": "Energierückgewinnung"}, {"value": "-334.4141388318348", "module": "D", "scenario": "Energierückgewinnung"}, {"value": "0.0", "module": "C1", "scenario": "Recycling"}, {"value": "1.43435960677528", "module": "C2", "scenario": "Recycling"}, {"value": "46.856475017669936", "module": "C3", "scenario": "Recycling"}, {"value": "0.0", "module": "C4", "scenario": "Recycling"}, {"value": "-17.490123997693914", "module": "D", "scenario": "Recycling"}, {"name": "referenceToUnitGroupDataSet", "value": {"shortDescription": [{"value": "MJ", "lang": "en"}], "type": "unit group data set", "refObjectId": "93a60a57-a3c8-11da-a746-0800200c9a66", "version": "03.00.000", "uri": "../unitgroups/93a60a57-a3c8-11da-a746-0800200c9a66.xml"}}]}, "flowProperties": [], "typeOfFlow": "Other flow", "classification": {"classHierarchy": "Größen / Umweltliche Größen / EPD EN 15804 / LCI Indikatoren", "name": "GaBiCategories"}}, {"dataSetInternalID": 4, "referenceToFlowDataSet": {"shortDescription": [{"value": "Use of non renewable primary energy (PENRE)", "lang": "en"}, {"value": "Nicht-erneuerbare Primärenergie als Energieträger (PENRE)", "lang": "de"}, {"value": "Uso de energía primaria no renovable, excluyendo los recursos de energía primaria no renovable utilizada como materia prima (PENRE)", "lang": "es"}], "type": "flow data set", "refObjectId": "ac857178-2b45-46ec-892a-a9a4332f0372", "version": "38.00.000", "uri": "../flows/ac857178-2b45-46ec-892a-a9a4332f0372.xml"}, "exchange direction": "INPUT", "meanAmount": 0.0, "other": {"anies": [{"value": "151.864257479548", "module": "A1-A3"}, {"value": "26.9676389812159", "module": "A4"}, {"value": "14.9246460619466", "module": "A5"}, {"value": "0.0", "module": "B1"}, {"value": "0.0", "module": "B2"}, {"value": "0.0", "module": "B3"}, {"value": "0.0", "module": "B4"}, {"value": "0.0", "module": "B5"}, {"value": "0.0", "module": "B6"}, {"value": "0.0", "module": "B7"}, {"value": "0.0", "module": "C1", "scenario": "Energierückgewinnung"}, {"value": "12.9609841691311", "module": "C2", "scenario": "Energierückgewinnung"}, {"value": "35.8198172411368", "module": "C3", "scenario": "Energierückgewinnung"}, {"value": "0.0", "module": "C4", "scenario": "Energierückgewinnung"}, {"value": "-819.4569810733027", "module": "D", "scenario": "Energierückgewinnung"}, {"value": "0.0", "module": "C1", "scenario": "Recycling"}, {"value": "12.9609841691311", "module": "C2", "scenario": "Recycling"}, {"value": "24.3479304534786", "module": "C3", "scenario": "Recycling"}, {"value": "0.0", "module": "C4", "scenario": "Recycling"}, {"value": "-441.42317640535475", "module": "D", "scenario": "Recycling"}, {"name": "referenceToUnitGroupDataSet", "value": {"shortDescription": [{"value": "MJ", "lang": "en"}], "type": "unit group data set", "refObjectId": "93a60a57-a3c8-11da-a746-0800200c9a66", "version": "03.00.000", "uri": "../unitgroups/93a60a57-a3c8-11da-a746-0800200c9a66.xml"}}]}, "flowProperties": [], "typeOfFlow": "Other flow", "classification": {"classHierarchy": "Quantities", "name": "GaBiCategories"}}, {"dataSetInternalID": 5, "referenceToFlowDataSet": {"shortDescription": [{"value": "Use of non renewable primary energy resources used as raw materials (PENRM)", "lang": "en"}, {"value": "Nicht-erneuerbare Primärenergie zur stofflichen Nutzung (PENRM)", "lang": "de"}, {"value": "Uso de la energía primaria no renovable utilizada como materia prima (PENRM)", "lang": "es"}], "type": "flow data set", "refObjectId": "1421caa0-679d-4bf4-b282-0eb850ccae27", "version": "38.00.000", "uri": "../flows/1421caa0-679d-4bf4-b282-0eb850ccae27.xml"}, "exchange direction": "INPUT", "meanAmount": 0.0, "other": {"anies": [{"value": "3.49375", "module": "A1-A3"}, {"value": "0.0", "module": "A4"}, {"value": "-3.49375", "module": "A5"}, {"value": "0.0", "module": "B1"}, {"value": "0.0", "module": "B2"}, {"value": "0.0", "module": "B3"}, {"value": "0.0", "module": "B4"}, {"value": "0.0", "module": "B5"}, {"value": "0.0", "module": "B6"}, {"value": "0.0", "module": "B7"}, {"value": "0.0", "module": "C1", "scenario": "Energierückgewinnung"}, {"value": "0.0", "module": "C2", "scenario": "Energierückgewinnung"}, {"value": "0.0", "module": "C3", "scenario": "Energierückgewinnung"}, {"value": "0.0", "module": "C4", "scenario": "Energierückgewinnung"}, {"value": "0.0", "module": "D", "scenario": "Energierückgewinnung"}, {"value": "0.0", "module": "C1", "scenario": "Recycling"}, {"value": "0.0", "module": "C2", "scenario": "Recycling"}, {"value": "0.0", "module": "C3", "scenario": "Recycling"}, {"value": "0.0", "module": "C4", "scenario": "Recycling"}, {"value": "0.0", "module": "D", "scenario": "Recycling"}, {"name": "referenceToUnitGroupDataSet", "value": {"shortDescription": [{"value": "MJ", "lang": "en"}], "type": "unit group data set", "refObjectId": "93a60a57-a3c8-11da-a746-0800200c9a66", "version": "03.00.000", "uri": "../unitgroups/93a60a57-a3c8-11da-a746-0800200c9a66.xml"}}]}, "flowProperties": [], "typeOfFlow": "Other flow", "classification": {"classHierarchy": "Quantities", "name": "GaBiCategories"}}, {"dataSetInternalID": 6, "referenceToFlowDataSet": {"shortDescription": [{"value": "Total use of non-renewable primary energy resources (PENRT)", "lang": "en"}, {"value": "Total nicht erneuerbare Primärenergie (PENRT)", "lang": "de"}, {"value": "Uso total de la energía primaria no renovable (energía primaria y recursos de energía primaria renovable utilizada como materia prima) (PENRT)", "lang": "es"}], "type": "flow data set", "refObjectId": "06159210-646b-4c8d-8583-da9b3b95a6c1", "version": "30.00.000", "uri": "../flows/06159210-646b-4c8d-8583-da9b3b95a6c1.xml"}, "exchange direction": "INPUT", "meanAmount": 0.0, "other": {"anies": [{"value": "155.358007479548", "module": "A1-A3"}, {"value": "26.9676389812159", "module": "A4"}, {"value": "11.4308960619466", "module": "A5"}, {"value": "0.0", "module": "B1"}, {"value": "0.0", "module": "B2"}, {"value": "0.0", "module": "B3"}, {"value": "0.0", "module": "B4"}, {"value": "0.0", "module": "B5"}, {"value": "0.0", "module": "B6"}, {"value": "0.0", "module": "B7"}, {"value": "0.0", "module": "C1", "scenario": "Energierückgewinnung"}, {"value": "12.9609841691311", "module": "C2", "scenario": "Energierückgewinnung"}, {"value": "35.8198172411368", "module": "C3", "scenario": "Energierückgewinnung"}, {"value": "0.0", "module": "C4", "scenario": "Energierückgewinnung"}, {"value": "-819.4569810733027", "module": "D", "scenario": "Energierückgewinnung"}, {"value": "0.0", "module": "C1", "scenario": "Recycling"}, {"value": "12.9609841691311", "module": "C2", "scenario": "Recycling"}, {"value": "24.3479304534786", "module": "C3", "scenario": "Recycling"}, {"value": "0.0", "module": "C4", "scenario": "Recycling"}, {"value": "-441.42317640535475", "module": "D", "scenario": "Recycling"}, {"name": "referenceToUnitGroupDataSet", "value": {"shortDescription": [{"value": "MJ", "lang": "en"}], "type": "unit group data set", "refObjectId": "93a60a57-a3c8-11da-a746-0800200c9a66", "version": "03.00.000", "uri": "../unitgroups/93a60a57-a3c8-11da-a746-0800200c9a66.xml"}}]}, "flowProperties": [], "typeOfFlow": "Other flow", "classification": {"classHierarchy": "Größen / Umweltliche Größen / EPD EN 15804 / LCI Indikatoren", "name": "GaBiCategories"}}, {"dataSetInternalID": 7, "referenceToFlowDataSet": {"shortDescription": [{"value": "Use of secondary material (SM)", "lang": "en"}, {"value": "Einsatz von Sekundärstoffen (SM)", "lang": "de"}, {"value": "Uso de materiales secundarios (SM)", "lang": "es"}], "type": "flow data set", "refObjectId": "c6a1f35f-2d09-4f54-8dfb-97e502e1ce92", "version": "30.00.000", "uri": "../flows/c6a1f35f-2d09-4f54-8dfb-97e502e1ce92.xml"}, "exchange direction": "INPUT", "meanAmount": 0.0, "other": {"anies": [{"value": "0.0", "module": "A1-A3"}, {"value": "0.0", "module": "A4"}, {"value": "0.0", "module": "A5"}, {"value": "0.0", "module": "B1"}, {"value": "0.0", "module": "B2"}, {"value": "0.0", "module": "B3"}, {"value": "0.0", "module": "B4"}, {"value": "0.0", "module": "B5"}, {"value": "0.0", "module": "B6"}, {"value": "0.0", "module": "B7"}, {"value": "0.0", "module": "C1", "scenario": "Energierückgewinnung"}, {"value": "0.0", "module": "C2", "scenario": "Energierückgewinnung"}, {"value": "0.0", "module": "C3", "scenario": "Energierückgewinnung"}, {"value": "0.0", "module": "C4", "scenario": "Energierückgewinnung"}, {"value": "0.0", "module": "D", "scenario": "Energierückgewinnung"}, {"value": "0.0", "module": "C1", "scenario": "Recycling"}, {"value": "0.0", "module": "C2", "scenario": "Recycling"}, {"value": "0.0", "module": "C3", "scenario": "Recycling"}, {"value": "0.0", "module": "C4", "scenario": "Recycling"}, {"value": "0.0", "module": "D", "scenario": "Recycling"}, {"name": "referenceToUnitGroupDataSet", "value": {"shortDescription": [{"value": "kg", "lang": "en"}], "type": "unit group data set", "refObjectId": "ad38d542-3fe9-439d-9b95-2f5f7752acaf", "version": "30.00.000", "uri": "../unitgroups/ad38d542-3fe9-439d-9b95-2f5f7752acaf.xml"}}]}, "flowProperties": [], "typeOfFlow": "Other flow", "classification": {"classHierarchy": "Größen / Umweltliche Größen / EPD EN 15804 / LCI Indikatoren", "name": "GaBiCategories"}}, {"dataSetInternalID": 8, "referenceToFlowDataSet": {"shortDescription": [{"value": "Use of renewable secondary fuels (RSF)", "lang": "en"}, {"value": "Erneuerbare Sekundärbrennstoffe (RSF)", "lang": "de"}, {"value": "Uso de combustibles secundarios renovables (RSF)", "lang": "es"}], "type": "flow data set", "refObjectId": "64333088-a55f-4aa2-9a31-c10b07816787", "version": "30.00.000", "uri": "../flows/64333088-a55f-4aa2-9a31-c10b07816787.xml"}, "exchange direction": "INPUT", "meanAmount": 0.0, "other": {"anies": [{"value": "0.0", "module": "A1-A3"}, {"value": "0.0", "module": "A4"}, {"value": "0.0", "module": "A5"}, {"value": "0.0", "module": "B1"}, {"value": "0.0", "module": "B2"}, {"value": "0.0", "module": "B3"}, {"value": "0.0", "module": "B4"}, {"value": "0.0", "module": "B5"}, {"value": "0.0", "module": "B6"}, {"value": "0.0", "module": "B7"}, {"value": "0.0", "module": "C1", "scenario": "Energierückgewinnung"}, {"value": "0.0", "module": "C2", "scenario": "Energierückgewinnung"}, {"value": "0.0", "module": "C3", "scenario": "Energierückgewinnung"}, {"value": "0.0", "module": "C4", "scenario": "Energierückgewinnung"}, {"value": "0.0", "module": "D", "scenario": "Energierückgewinnung"}, {"value": "0.0", "module": "C1", "scenario": "Recycling"}, {"value": "0.0", "module": "C2", "scenario": "Recycling"}, {"value": "0.0", "module": "C3", "scenario": "Recycling"}, {"value": "0.0", "module": "C4", "scenario": "Recycling"}, {"value": "0.0", "module": "D", "scenario": "Recycling"}, {"name": "referenceToUnitGroupDataSet", "value": {"shortDescription": [{"value": "MJ", "lang": "en"}], "type": "unit group data set", "refObjectId": "93a60a57-a3c8-11da-a746-0800200c9a66", "version": "03.00.000", "uri": "../unitgroups/93a60a57-a3c8-11da-a746-0800200c9a66.xml"}}]}, "flowProperties": [], "typeOfFlow": "Other flow", "classification": {"classHierarchy": "Größen / Umweltliche Größen / EPD EN 15804 / LCI Indikatoren", "name": "GaBiCategories"}}, {"dataSetInternalID": 9, "referenceToFlowDataSet": {"shortDescription": [{"value": "Use of non renewable secondary fuels (NRSF)", "lang": "en"}, {"value": "Nicht erneuerbare Sekundärbrennstoffe (NRSF)", "lang": "de"}, {"value": "Uso de combustibles secundarios no renovables (NRSF)", "lang": "es"}], "type": "flow data set", "refObjectId": "89def144-d39a-4287-b86f-efde453ddcb2", "version": "30.00.000", "uri": "../flows/89def144-d39a-4287-b86f-efde453ddcb2.xml"}, "exchange direction": "INPUT", "meanAmount": 0.0, "other": {"anies": [{"value": "0.0", "module": "A1-A3"}, {"value": "0.0", "module": "A4"}, {"value": "0.0", "module": "A5"}, {"value": "0.0", "module": "B1"}, {"value": "0.0", "module": "B2"}, {"value": "0.0", "module": "B3"}, {"value": "0.0", "module": "B4"}, {"value": "0.0", "module": "B5"}, {"value": "0.0", "module": "B6"}, {"value": "0.0", "module": "B7"}, {"value": "0.0", "module": "C1", "scenario": "Energierückgewinnung"}, {"value": "0.0", "module": "C2", "scenario": "Energierückgewinnung"}, {"value": "0.0", "module": "C3", "scenario": "Energierückgewinnung"}, {"value": "0.0", "module": "C4", "scenario": "Energierückgewinnung"}, {"value": "0.0", "module": "D", "scenario": "Energierückgewinnung"}, {"value": "0.0", "module": "C1", "scenario": "Recycling"}, {"value": "0.0", "module": "C2", "scenario": "Recycling"}, {"value": "0.0", "module": "C3", "scenario": "Recycling"}, {"value": "0.0", "module": "C4", "scenario": "Recycling"}, {"value": "0.0", "module": "D", "scenario": "Recycling"}, {"name": "referenceToUnitGroupDataSet", "value": {"shortDescription": [{"value": "MJ", "lang": "en"}], "type": "unit group data set", "refObjectId": "93a60a57-a3c8-11da-a746-0800200c9a66", "version": "03.00.000", "uri": "../unitgroups/93a60a57-a3c8-11da-a746-0800200c9a66.xml"}}]}, "flowProperties": [], "typeOfFlow": "Other flow", "classification": {"classHierarchy": "Größen / Umweltliche Größen / EPD EN 15804 / LCI Indikatoren", "name": "GaBiCategories"}}, {"dataSetInternalID": 10, "referenceToFlowDataSet": {"shortDescription": [{"value": "Use of net fresh water (FW)", "lang": "en"}, {"value": "Einsatz von Süßwasserressourcen (FW)", "lang": "de"}, {"value": "Uso neto de recursos de agua dulce (FW)", "lang": "es"}], "type": "flow data set", "refObjectId": "3cf952c8-f3a4-461d-8c96-96456ca62246", "version": "30.00.000", "uri": "../flows/3cf952c8-f3a4-461d-8c96-96456ca62246.xml"}, "exchange direction": "INPUT", "meanAmount": 0.0, "other": {"anies": [{"value": "0.379351663057208", "module": "A1-A3"}, {"value": "0.00278811264387936", "module": "A4"}, {"value": "0.039070188748459", "module": "A5"}, {"value": "0.0", "module": "B1"}, {"value": "0.0", "module": "B2"}, {"value": "0.0", "module": "B3"}, {"value": "0.0", "module": "B4"}, {"value": "0.0", "module": "B5"}, {"value": "0.0", "module": "B6"}, {"value": "0.0", "module": "B7"}, {"value": "0.0", "module": "C1", "scenario": "Energierückgewinnung"}, {"value": "0.0013400017652359", "module": "C2", "scenario": "Energierückgewinnung"}, {"value": "0.386432081919239", "module": "C3", "scenario": "Energierückgewinnung"}, {"value": "0.0", "module": "C4", "scenario": "Energierückgewinnung"}, {"value": "-0.10646232650189785", "module": "D", "scenario": "Energierückgewinnung"}, {"value": "0.0", "module": "C1", "scenario": "Recycling"}, {"value": "0.0013400017652359", "module": "C2", "scenario": "Recycling"}, {"value": "0.0118878011162682", "module": "C3", "scenario": "Recycling"}, {"value": "0.0", "module": "C4", "scenario": "Recycling"}, {"value": "-0.00640823808413704", "module": "D", "scenario": "Recycling"}, {"name": "referenceToUnitGroupDataSet", "value": {"shortDescription": [{"value": "m3", "lang": "en"}], "type": "unit group data set", "refObjectId": "cd950537-0a98-4044-9ba7-9f9a68d0a504", "version": "30.00.000", "uri": "../unitgroups/cd950537-0a98-4044-9ba7-9f9a68d0a504.xml"}}]}, "flowProperties": [], "typeOfFlow": "Other flow", "classification": {"classHierarchy": "Größen / Umweltliche Größen / EPD EN 15804 / LCI Indikatoren", "name": "GaBiCategories"}}, {"dataSetInternalID": 11, "referenceToFlowDataSet": {"shortDescription": [{"value": "Hazardous waste disposed (HWD)", "lang": "en"}, {"value": "Gefährlicher Abfall zur Deponie (HWD)", "lang": "de"}, {"value": "Residuos peligrosos eliminados (HWD)", "lang": "es"}], "type": "flow data set", "refObjectId": "430f9e0f-59b2-46a0-8e0d-55e0e84948fc", "version": "30.00.000", "uri": "../flows/430f9e0f-59b2-46a0-8e0d-55e0e84948fc.xml"}, "exchange direction": "OUTPUT", "meanAmount": 0.0, "other": {"anies": [{"value": "1.75030343217634E-8", "module": "A1-A3"}, {"value": "1.31289532081322E-9", "module": "A4"}, {"value": "2.42717927945946E-9", "module": "A5"}, {"value": "0.0", "module": "B1"}, {"value": "0.0", "module": "B2"}, {"value": "0.0", "module": "B3"}, {"value": "0.0", "module": "B4"}, {"value": "0.0", "module": "B5"}, {"value": "0.0", "module": "B6"}, {"value": "0.0", "module": "B7"}, {"value": "0.0", "module": "C1", "scenario": "Energierückgewinnung"}, {"value": "6.30993891628376E-10", "module": "C2", "scenario": "Energierückgewinnung"}, {"value": "2.85325670440887E-8", "module": "C3", "scenario": "Energierückgewinnung"}, {"value": "0.0", "module": "C4", "scenario": "Energierückgewinnung"}, {"value": "-7.763222327411914E-7", "module": "D", "scenario": "Energierückgewinnung"}, {"value": "0.0", "module": "C1", "scenario": "Recycling"}, {"value": "6.30993891628376E-10", "module": "C2", "scenario": "Recycling"}, {"value": "5.78880966321102E-8", "module": "C3", "scenario": "Recycling"}, {"value": "0.0", "module": "C4", "scenario": "Recycling"}, {"value": "-4.5965472563580545E-8", "module": "D", "scenario": "Recycling"}, {"name": "referenceToUnitGroupDataSet", "value": {"shortDescription": [{"value": "kg", "lang": "en"}], "type": "unit group data set", "refObjectId": "ad38d542-3fe9-439d-9b95-2f5f7752acaf", "version": "30.00.000", "uri": "../unitgroups/ad38d542-3fe9-439d-9b95-2f5f7752acaf.xml"}}]}, "flowProperties": [], "typeOfFlow": "Other flow", "classification": {"classHierarchy": "Größen / Umweltliche Größen / EPD EN 15804 / LCI Indikatoren", "name": "GaBiCategories"}}, {"dataSetInternalID": 12, "referenceToFlowDataSet": {"shortDescription": [{"value": "Non-hazardous waste disposed (NHWD)", "lang": "en"}, {"value": "Entsorgter nicht gefährlicher Abfall (NHWD)", "lang": "de"}, {"value": "Residuos no peligrosos eliminados (NHWD)", "lang": "es"}], "type": "flow data set", "refObjectId": "b29ef66b-e286-4afa-949f-62f1a7b4d7fa", "version": "30.00.000", "uri": "../flows/b29ef66b-e286-4afa-949f-62f1a7b4d7fa.xml"}, "exchange direction": "OUTPUT", "meanAmount": 0.0, "other": {"anies": [{"value": "0.0960878590211478", "module": "A1-A3"}, {"value": "0.00455961964639166", "module": "A4"}, {"value": "0.0611284285442448", "module": "A5"}, {"value": "0.0", "module": "B1"}, {"value": "0.0", "module": "B2"}, {"value": "0.0", "module": "B3"}, {"value": "0.0", "module": "B4"}, {"value": "0.0", "module": "B5"}, {"value": "0.0", "module": "B6"}, {"value": "0.0", "module": "B7"}, {"value": "0.0", "module": "C1", "scenario": "Energierückgewinnung"}, {"value": "0.0021914101599812", "module": "C2", "scenario": "Energierückgewinnung"}, {"value": "1.09811401238985", "module": "C3", "scenario": "Energierückgewinnung"}, {"value": "0.0", "module": "C4", "scenario": "Energierückgewinnung"}, {"value": "-0.4672453794780029", "module": "D", "scenario": "Energierückgewinnung"}, {"value": "0.0", "module": "C1", "scenario": "Recycling"}, {"value": "0.0021914101599812", "module": "C2", "scenario": "Recycling"}, {"value": "0.0397584135814224", "module": "C3", "scenario": "Recycling"}, {"value": "0.0", "module": "C4", "scenario": "Recycling"}, {"value": "-0.0953161006819325", "module": "D", "scenario": "Recycling"}, {"name": "referenceToUnitGroupDataSet", "value": {"shortDescription": [{"value": "kg", "lang": "en"}], "type": "unit group data set", "refObjectId": "ad38d542-3fe9-439d-9b95-2f5f7752acaf", "version": "30.00.000", "uri": "../unitgroups/ad38d542-3fe9-439d-9b95-2f5f7752acaf.xml"}}]}, "flowProperties": [], "typeOfFlow": "Other flow", "classification": {"classHierarchy": "Größen / Umweltliche Größen / EPD EN 15804 / LCI Indikatoren", "name": "GaBiCategories"}}, {"dataSetInternalID": 13, "referenceToFlowDataSet": {"shortDescription": [{"value": "Radioactive waste disposed (RWD)", "lang": "en"}, {"value": "Entsorgter radioaktiver Abfall (RWD)", "lang": "de"}, {"value": "Residuos radiactivos eliminados (RWD)", "lang": "es"}], "type": "flow data set", "refObjectId": "3449546e-52ad-4b39-b809-9fb77cea8ff6", "version": "30.00.000", "uri": "../flows/3449546e-52ad-4b39-b809-9fb77cea8ff6.xml"}, "exchange direction": "OUTPUT", "meanAmount": 0.0, "other": {"anies": [{"value": "0.00133804908036466", "module": "A1-A3"}, {"value": "4.29235351877091E-5", "module": "A4"}, {"value": "1.26019029581343E-4", "module": "A5"}, {"value": "0.0", "module": "B1"}, {"value": "0.0", "module": "B2"}, {"value": "0.0", "module": "B3"}, {"value": "0.0", "module": "B4"}, {"value": "0.0", "module": "B5"}, {"value": "0.0", "module": "B6"}, {"value": "0.0", "module": "B7"}, {"value": "0.0", "module": "C1", "scenario": "Energierückgewinnung"}, {"value": "2.06295872040763E-5", "module": "C2", "scenario": "Energierückgewinnung"}, {"value": "0.00109715179506964", "module": "C3", "scenario": "Energierückgewinnung"}, {"value": "0.0", "module": "C4", "scenario": "Energierückgewinnung"}, {"value": "-0.02983637570440815", "module": "D", "scenario": "Energierückgewinnung"}, {"value": "0.0", "module": "C1", "scenario": "Recycling"}, {"value": "2.06295872040763E-5", "module": "C2", "scenario": "Recycling"}, {"value": "0.00224599124206395", "module": "C3", "scenario": "Recycling"}, {"value": "0.0", "module": "C4", "scenario": "Recycling"}, {"value": "-0.001536354975609427", "module": "D", "scenario": "Recycling"}, {"name": "referenceToUnitGroupDataSet", "value": {"shortDescription": [{"value": "kg", "lang": "en"}], "type": "unit group data set", "refObjectId": "ad38d542-3fe9-439d-9b95-2f5f7752acaf", "version": "30.00.000", "uri": "../unitgroups/ad38d542-3fe9-439d-9b95-2f5f7752acaf.xml"}}]}, "flowProperties": [], "typeOfFlow": "Other flow", "classification": {"classHierarchy": "Größen / Umweltliche Größen / EPD EN 15804 / LCI Indikatoren", "name": "GaBiCategories"}}, {"dataSetInternalID": 14, "referenceToFlowDataSet": {"shortDescription": [{"value": "Components for re-use (CRU)", "lang": "en"}, {"value": "Komponenten für die Wiederverwendung (CRU)", "lang": "de"}, {"value": "Componentes para su reutilización (CRU)", "lang": "es"}], "type": "flow data set", "refObjectId": "a2b32f97-3fc7-4af2-b209-525bc6426f33", "version": "30.00.000", "uri": "../flows/a2b32f97-3fc7-4af2-b209-525bc6426f33.xml"}, "exchange direction": "OUTPUT", "meanAmount": 0.0, "other": {"anies": [{"value": "0.0", "module": "A1-A3"}, {"value": "0.0", "module": "A4"}, {"value": "0.0", "module": "A5"}, {"value": "0.0", "module": "B1"}, {"value": "0.0", "module": "B2"}, {"value": "0.0", "module": "B3"}, {"value": "0.0", "module": "B4"}, {"value": "0.0", "module": "B5"}, {"value": "0.0", "module": "B6"}, {"value": "0.0", "module": "B7"}, {"value": "0.0", "module": "C1", "scenario": "Energierückgewinnung"}, {"value": "0.0", "module": "C2", "scenario": "Energierückgewinnung"}, {"value": "0.0", "module": "C3", "scenario": "Energierückgewinnung"}, {"value": "0.0", "module": "C4", "scenario": "Energierückgewinnung"}, {"value": "0.0", "module": "D", "scenario": "Energierückgewinnung"}, {"value": "0.0", "module": "C1", "scenario": "Recycling"}, {"value": "0.0", "module": "C2", "scenario": "Recycling"}, {"value": "0.0", "module": "C3", "scenario": "Recycling"}, {"value": "0.0", "module": "C4", "scenario": "Recycling"}, {"value": "0.0", "module": "D", "scenario": "Recycling"}, {"name": "referenceToUnitGroupDataSet", "value": {"shortDescription": [{"value": "kg", "lang": "en"}], "type": "unit group data set", "refObjectId": "ad38d542-3fe9-439d-9b95-2f5f7752acaf", "version": "30.00.000", "uri": "../unitgroups/ad38d542-3fe9-439d-9b95-2f5f7752acaf.xml"}}]}, "flowProperties": [], "typeOfFlow": "Other flow", "classification": {"classHierarchy": "Größen / Umweltliche Größen / EPD EN 15804 / LCI Indikatoren", "name": "GaBiCategories"}}, {"dataSetInternalID": 15, "referenceToFlowDataSet": {"shortDescription": [{"value": "Materials for recycling (MFR)", "lang": "en"}, {"value": "Stoffe zum Recycling (MFR)", "lang": "de"}, {"value": "Materiales para el reciclaje (MFR)", "lang": "es"}], "type": "flow data set", "refObjectId": "d7fe48a5-4103-49c8-9aae-b0b5dfdbd6ae", "version": "30.00.000", "uri": "../flows/d7fe48a5-4103-49c8-9aae-b0b5dfdbd6ae.xml"}, "exchange direction": "OUTPUT", "meanAmount": 0.0, "other": {"anies": [{"value": "0.0", "module": "A1-A3"}, {"value": "0.0", "module": "A4"}, {"value": "0.0", "module": "A5"}, {"value": "0.0", "module": "B1"}, {"value": "0.0", "module": "B2"}, {"value": "0.0", "module": "B3"}, {"value": "0.0", "module": "B4"}, {"value": "0.0", "module": "B5"}, {"value": "0.0", "module": "B6"}, {"value": "0.0", "module": "B7"}, {"value": "0.0", "module": "C1", "scenario": "Energierückgewinnung"}, {"value": "0.0", "module": "C2", "scenario": "Energierückgewinnung"}, {"value": "0.0", "module": "C3", "scenario": "Energierückgewinnung"}, {"value": "0.0", "module": "C4", "scenario": "Energierückgewinnung"}, {"value": "0.0", "module": "D", "scenario": "Energierückgewinnung"}, {"value": "0.0", "module": "C1", "scenario": "Recycling"}, {"value": "0.0", "module": "C2", "scenario": "Recycling"}, {"value": "0.0", "module": "C3", "scenario": "Recycling"}, {"value": "0.0", "module": "C4", "scenario": "Recycling"}, {"value": "0.0", "module": "D", "scenario": "Recycling"}, {"name": "referenceToUnitGroupDataSet", "value": {"shortDescription": [{"value": "kg", "lang": "en"}], "type": "unit group data set", "refObjectId": "ad38d542-3fe9-439d-9b95-2f5f7752acaf", "version": "30.00.000", "uri": "../unitgroups/ad38d542-3fe9-439d-9b95-2f5f7752acaf.xml"}}]}, "flowProperties": [], "typeOfFlow": "Other flow", "classification": {"classHierarchy": "Größen / Umweltliche Größen / EPD EN 15804 / LCI Indikatoren", "name": "GaBiCategories"}}, {"dataSetInternalID": 16, "referenceToFlowDataSet": {"shortDescription": [{"value": "Materials for energy recovery (MER)", "lang": "en"}, {"value": "Stoffe für die Energierückgewinnung (MER)", "lang": "de"}, {"value": "Materiales para valorización energética (recuperación de energía) (MER)", "lang": "es"}], "type": "flow data set", "refObjectId": "59a9181c-3aaf-46ee-8b13-2b3723b6e447", "version": "30.00.000", "uri": "../flows/59a9181c-3aaf-46ee-8b13-2b3723b6e447.xml"}, "exchange direction": "OUTPUT", "meanAmount": 0.0, "other": {"anies": [{"value": "0.0", "module": "A1-A3"}, {"value": "0.0", "module": "A4"}, {"value": "0.0", "module": "A5"}, {"value": "0.0", "module": "B1"}, {"value": "0.0", "module": "B2"}, {"value": "0.0", "module": "B3"}, {"value": "0.0", "module": "B4"}, {"value": "0.0", "module": "B5"}, {"value": "0.0", "module": "B6"}, {"value": "0.0", "module": "B7"}, {"value": "0.0", "module": "C1", "scenario": "Energierückgewinnung"}, {"value": "0.0", "module": "C2", "scenario": "Energierückgewinnung"}, {"value": "0.0", "module": "C3", "scenario": "Energierückgewinnung"}, {"value": "0.0", "module": "C4", "scenario": "Energierückgewinnung"}, {"value": "0.0", "module": "D", "scenario": "Energierückgewinnung"}, {"value": "0.0", "module": "C1", "scenario": "Recycling"}, {"value": "0.0", "module": "C2", "scenario": "Recycling"}, {"value": "7.375313209346491", "module": "C3", "scenario": "Recycling"}, {"value": "0.0", "module": "C4", "scenario": "Recycling"}, {"value": "0.0", "module": "D", "scenario": "Recycling"}, {"name": "referenceToUnitGroupDataSet", "value": {"shortDescription": [{"value": "kg", "lang": "en"}], "type": "unit group data set", "refObjectId": "ad38d542-3fe9-439d-9b95-2f5f7752acaf", "version": "30.00.000", "uri": "../unitgroups/ad38d542-3fe9-439d-9b95-2f5f7752acaf.xml"}}]}, "flowProperties": [], "typeOfFlow": "Other flow", "classification": {"classHierarchy": "Größen / Umweltliche Größen / EPD EN 15804 / LCI Indikatoren", "name": "GaBiCategories"}}, {"dataSetInternalID": 17, "referenceToFlowDataSet": {"shortDescription": [{"value": "Exported electrical energy (EEE)", "lang": "en"}, {"value": "Exportierte elektrische Energie (EEE)", "lang": "de"}, {"value": "Energía exportada electrica (EEE)", "lang": "es"}], "type": "flow data set", "refObjectId": "4da0c987-2b76-40d6-9e9e-82a017aaaf29", "version": "30.00.000", "uri": "../flows/4da0c987-2b76-40d6-9e9e-82a017aaaf29.xml"}, "exchange direction": "OUTPUT", "meanAmount": 0.0, "other": {"anies": [{"value": "0.0", "module": "A1-A3"}, {"value": "0.0", "module": "A4"}, {"value": "9.78829240131826", "module": "A5"}, {"value": "0.0", "module": "B1"}, {"value": "0.0", "module": "B2"}, {"value": "0.0", "module": "B3"}, {"value": "0.0", "module": "B4"}, {"value": "0.0", "module": "B5"}, {"value": "0.0", "module": "B6"}, {"value": "0.0", "module": "B7"}, {"value": "0.0", "module": "C1", "scenario": "Energierückgewinnung"}, {"value": "0.0", "module": "C2", "scenario": "Energierückgewinnung"}, {"value": "186.064010300406", "module": "C3", "scenario": "Energierückgewinnung"}, {"value": "0.0", "module": "C4", "scenario": "Energierückgewinnung"}, {"value": "0.0", "module": "D", "scenario": "Energierückgewinnung"}, {"value": "0.0", "module": "C1", "scenario": "Recycling"}, {"value": "0.0", "module": "C2", "scenario": "Recycling"}, {"value": "0.0", "module": "C3", "scenario": "Recycling"}, {"value": "0.0", "module": "C4", "scenario": "Recycling"}, {"value": "0.0", "module": "D", "scenario": "Recycling"}, {"name": "referenceToUnitGroupDataSet", "value": {"shortDescription": [{"value": "MJ", "lang": "en"}], "type": "unit group data set", "refObjectId": "93a60a57-a3c8-11da-a746-0800200c9a66", "version": "03.00.000", "uri": "../unitgroups/93a60a57-a3c8-11da-a746-0800200c9a66.xml"}}]}, "flowProperties": [], "typeOfFlow": "Other flow", "classification": {"classHierarchy": "Größen / Umweltliche Größen / EPD EN 15804 / LCI Indikatoren", "name": "GaBiCategories"}}, {"dataSetInternalID": 18, "referenceToFlowDataSet": {"shortDescription": [{"value": "Exported thermal energy (EET)", "lang": "en"}, {"value": "Exportierte thermische Energie (EET)", "lang": "de"}, {"value": "Energía exportada termal (EET)", "lang": "es"}], "type": "flow data set", "refObjectId": "98daf38a-7a79-46d3-9a37-2b7bd0955810", "version": "30.00.000", "uri": "../flows/98daf38a-7a79-46d3-9a37-2b7bd0955810.xml"}, "exchange direction": "OUTPUT", "meanAmount": 0.0, "other": {"anies": [{"value": "0.0", "module": "A1-A3"}, {"value": "0.0", "module": "A4"}, {"value": "22.9280273000297", "module": "A5"}, {"value": "0.0", "module": "B1"}, {"value": "0.0", "module": "B2"}, {"value": "0.0", "module": "B3"}, {"value": "0.0", "module": "B4"}, {"value": "0.0", "module": "B5"}, {"value": "0.0", "module": "B6"}, {"value": "0.0", "module": "B7"}, {"value": "0.0", "module": "C1", "scenario": "Energierückgewinnung"}, {"value": "0.0", "module": "C2", "scenario": "Energierückgewinnung"}, {"value": "436.215784631989", "module": "C3", "scenario": "Energierückgewinnung"}, {"value": "0.0", "module": "C4", "scenario": "Energierückgewinnung"}, {"value": "0.0", "module": "D", "scenario": "Energierückgewinnung"}, {"value": "0.0", "module": "C1", "scenario": "Recycling"}, {"value": "0.0", "module": "C2", "scenario": "Recycling"}, {"value": "0.0", "module": "C3", "scenario": "Recycling"}, {"value": "0.0", "module": "C4", "scenario": "Recycling"}, {"value": "0.0", "module": "D", "scenario": "Recycling"}, {"name": "referenceToUnitGroupDataSet", "value": {"shortDescription": [{"value": "MJ", "lang": "en"}], "type": "unit group data set", "refObjectId": "93a60a57-a3c8-11da-a746-0800200c9a66", "version": "03.00.000", "uri": "../unitgroups/93a60a57-a3c8-11da-a746-0800200c9a66.xml"}}]}, "flowProperties": [], "typeOfFlow": "Other flow", "classification": {"classHierarchy": "Größen / Umweltliche Größen / EPD EN 15804 / LCI Indikatoren", "name": "GaBiCategories"}}]}, "LCIAResults": {"LCIAResult": [{"referenceToLCIAMethodDataSet": {"shortDescription": [{"value": "Global Warming Potential - total (GWP-total)", "lang": "en"}, {"value": "Globales Erwärmungspotenzial - total (GWP-total)", "lang": "de"}], "type": "LCIA method data set", "refObjectId": "a7ea142a-9749-11ed-a8fc-0242ac120002", "version": "04.00.017", "uri": "../lciamethods/a7ea142a-9749-11ed-a8fc-0242ac120002.xml"}, "meanAmount": 0.0, "other": {"anies": [{"value": "-129.384758474953", "module": "A1-A3"}, {"value": "2.10348944031878", "module": "A4"}, {"value": "1.5470417978189062", "module": "A5"}, {"value": "0.0", "module": "B1"}, {"value": "0.0", "module": "B2"}, {"value": "0.0", "module": "B3"}, {"value": "0.0", "module": "B4"}, {"value": "0.0", "module": "B5"}, {"value": "0.0", "module": "B6"}, {"value": "0.0", "module": "B7"}, {"value": "0.0", "module": "C1", "scenario": "Energierückgewinnung"}, {"value": "1.0094851806642477", "module": "C2", "scenario": "Energierückgewinnung"}, {"value": "151.8598598696679", "module": "C3", "scenario": "Energierückgewinnung"}, {"value": "0.0", "module": "C4", "scenario": "Energierückgewinnung"}, {"value": "-54.48275121686296", "module": "D", "scenario": "Energierückgewinnung"}, {"value": "0.0", "module": "C1", "scenario": "Recycling"}, {"value": "1.0094851806642477", "module": "C2", "scenario": "Recycling"}, {"value": "150.42148814026632", "module": "C3", "scenario": "Recycling"}, {"value": "0.0", "module": "C4", "scenario": "Recycling"}, {"value": "-7.50468047419584", "module": "D", "scenario": "Recycling"}, {"name": "referenceToUnitGroupDataSet", "value": {"shortDescription": [{"value": "kg CO2-eq.", "lang": "en"}], "type": "unit group data set", "refObjectId": "1ebf3012-d0db-4de2-aefd-ef30cedb0be1", "version": "30.00.000", "uri": "../unitgroups/1ebf3012-d0db-4de2-aefd-ef30cedb0be1.xml"}}]}}, {"referenceToLCIAMethodDataSet": {"shortDescription": [{"value": "Global Warming Potential - fossil fuels (GWP-fossil)", "lang": "en"}, {"value": "Globales Erwärmungspotenzial - fossil (GWP-fossil)", "lang": "de"}], "type": "LCIA method data set", "refObjectId": "a7ea19c0-9749-11ed-a8fc-0242ac120002", "version": "01.00.009", "uri": "../lciamethods/a7ea19c0-9749-11ed-a8fc-0242ac120002.xml"}, "meanAmount": 0.0, "other": {"anies": [{"value": "18.4935067097017", "module": "A1-A3"}, {"value": "2.05223401417397", "module": "A4"}, {"value": "1.47038200767865", "module": "A5"}, {"value": "0.0", "module": "B1"}, {"value": "0.0", "module": "B2"}, {"value": "0.0", "module": "B3"}, {"value": "0.0", "module": "B4"}, {"value": "0.0", "module": "B5"}, {"value": "0.0", "module": "B6"}, {"value": "0.0", "module": "B7"}, {"value": "0.0", "module": "C1", "scenario": "Energierückgewinnung"}, {"value": "0.984851180673695", "module": "C2", "scenario": "Energierückgewinnung"}, {"value": "2.52496711509294", "module": "C3", "scenario": "Energierückgewinnung"}, {"value": "0.0", "module": "C4", "scenario": "Energierückgewinnung"}, {"value": "-54.098626182327365", "module": "D", "scenario": "Energierückgewinnung"}, {"value": "0.0", "module": "C1", "scenario": "Recycling"}, {"value": "0.984851180673695", "module": "C2", "scenario": "Recycling"}, {"value": "2.17783327384817", "module": "C3", "scenario": "Recycling"}, {"value": "0.0", "module": "C4", "scenario": "Recycling"}, {"value": "-7.43100355862202", "module": "D", "scenario": "Recycling"}, {"name": "referenceToUnitGroupDataSet", "value": {"shortDescription": [{"value": "kg CO2-eq.", "lang": "en"}], "type": "unit group data set", "refObjectId": "1ebf3012-d0db-4de2-aefd-ef30cedb0be1", "version": "30.00.000", "uri": "../unitgroups/1ebf3012-d0db-4de2-aefd-ef30cedb0be1.xml"}}]}}, {"referenceToLCIAMethodDataSet": {"shortDescription": [{"value": "Global Warming Potential - biogenic (GWP-biogenic)", "lang": "en"}, {"value": "Globales Erwärmungspotenzial - biogen (GWP-biogenic)", "lang": "de"}], "type": "LCIA method data set", "refObjectId": "a7ea186c-9749-11ed-a8fc-0242ac120002", "version": "01.00.006", "uri": "../lciamethods/a7ea186c-9749-11ed-a8fc-0242ac120002.xml"}, "meanAmount": 0.0, "other": {"anies": [{"value": "-148.242555829259", "module": "A1-A3"}, {"value": "0.0117507534501994", "module": "A4"}, {"value": "0.055466462653192994", "module": "A5"}, {"value": "0.0", "module": "B1"}, {"value": "0.0", "module": "B2"}, {"value": "0.0", "module": "B3"}, {"value": "0.0", "module": "B4"}, {"value": "0.0", "module": "B5"}, {"value": "0.0", "module": "B6"}, {"value": "0.0", "module": "B7"}, {"value": "0.0", "module": "C1", "scenario": "Energierückgewinnung"}, {"value": "0.00564756080845744", "module": "C2", "scenario": "Energierückgewinnung"}, {"value": "149.334145674849", "module": "C3", "scenario": "Energierückgewinnung"}, {"value": "0.0", "module": "C4", "scenario": "Energierückgewinnung"}, {"value": "-0.37762778707226746", "module": "D", "scenario": "Energierückgewinnung"}, {"value": "0.0", "module": "C1", "scenario": "Recycling"}, {"value": "0.00564756080845744", "module": "C2", "scenario": "Recycling"}, {"value": "148.242555829259", "module": "C3", "scenario": "Recycling"}, {"value": "0.0", "module": "C4", "scenario": "Recycling"}, {"value": "-0.0716659967199031", "module": "D", "scenario": "Recycling"}, {"name": "referenceToUnitGroupDataSet", "value": {"shortDescription": [{"value": "kg CO2-eq.", "lang": "en"}], "type": "unit group data set", "refObjectId": "1ebf3012-d0db-4de2-aefd-ef30cedb0be1", "version": "30.00.000", "uri": "../unitgroups/1ebf3012-d0db-4de2-aefd-ef30cedb0be1.xml"}}]}}, {"referenceToLCIAMethodDataSet": {"shortDescription": [{"value": "Global Warming Potential - land use and land use change (GWP-luluc)", "lang": "en"}, {"value": "Globales Erwärmungspotenzial - luluc (GWP-luluc)", "lang": "de"}], "type": "LCIA method data set", "refObjectId": "a7ea1ae2-9749-11ed-a8fc-0242ac120002", "version": "01.00.006", "uri": "../lciamethods/a7ea1ae2-9749-11ed-a8fc-0242ac120002.xml"}, "meanAmount": 0.0, "other": {"anies": [{"value": "0.364290644604303", "module": "A1-A3"}, {"value": "0.0395046726946106", "module": "A4"}, {"value": "0.021193327487063", "module": "A5"}, {"value": "0.0", "module": "B1"}, {"value": "0.0", "module": "B2"}, {"value": "0.0", "module": "B3"}, {"value": "0.0", "module": "B4"}, {"value": "0.0", "module": "B5"}, {"value": "0.0", "module": "B6"}, {"value": "0.0", "module": "B7"}, {"value": "0.0", "module": "C1", "scenario": "Energierückgewinnung"}, {"value": "0.0189864391820952", "module": "C2", "scenario": "Energierückgewinnung"}, {"value": "7.47079725950942E-4", "module": "C3", "scenario": "Energierückgewinnung"}, {"value": "0.0", "module": "C4", "scenario": "Energierückgewinnung"}, {"value": "-0.006497247463329321", "module": "D", "scenario": "Energierückgewinnung"}, {"value": "0.0", "module": "C1", "scenario": "Recycling"}, {"value": "0.0189864391820952", "module": "C2", "scenario": "Recycling"}, {"value": "0.00109903715915114", "module": "C3", "scenario": "Recycling"}, {"value": "0.0", "module": "C4", "scenario": "Recycling"}, {"value": "-0.002010918853918162", "module": "D", "scenario": "Recycling"}, {"name": "referenceToUnitGroupDataSet", "value": {"shortDescription": [{"value": "kg CO2-eq.", "lang": "en"}], "type": "unit group data set", "refObjectId": "1ebf3012-d0db-4de2-aefd-ef30cedb0be1", "version": "30.00.000", "uri": "../unitgroups/1ebf3012-d0db-4de2-aefd-ef30cedb0be1.xml"}}]}}, {"referenceToLCIAMethodDataSet": {"shortDescription": [{"value": "Depletion potential of the stratospheric ozone layer (ODP)", "lang": "en"}, {"value": "Abbaupotenzial der stratosphärischen Ozonschicht (ODP)", "lang": "de"}], "type": "LCIA method data set", "refObjectId": "b5c629d6-def3-11e6-bf01-fe55135034f3", "version": "02.00.013", "uri": "../lciamethods/b5c629d6-def3-11e6-bf01-fe55135034f3.xml"}, "meanAmount": 0.0, "other": {"anies": [{"value": "1.05954011453912E-11", "module": "A1-A3"}, {"value": "6.4856735262374E-13", "module": "A4"}, {"value": "1.87537347153451E-12", "module": "A5"}, {"value": "0.0", "module": "B1"}, {"value": "0.0", "module": "B2"}, {"value": "0.0", "module": "B3"}, {"value": "0.0", "module": "B4"}, {"value": "0.0", "module": "B5"}, {"value": "0.0", "module": "B6"}, {"value": "0.0", "module": "B7"}, {"value": "0.0", "module": "C1", "scenario": "Energierückgewinnung"}, {"value": "3.11709571454393E-13", "module": "C2", "scenario": "Energierückgewinnung"}, {"value": "2.54531507701472E-11", "module": "C3", "scenario": "Energierückgewinnung"}, {"value": "0.0", "module": "C4", "scenario": "Energierückgewinnung"}, {"value": "-6.959261132531976E-10", "module": "D", "scenario": "Energierückgewinnung"}, {"value": "0.0", "module": "C1", "scenario": "Recycling"}, {"value": "3.11709571454393E-13", "module": "C2", "scenario": "Recycling"}, {"value": "5.24203213665295E-11", "module": "C3", "scenario": "Recycling"}, {"value": "0.0", "module": "C4", "scenario": "Recycling"}, {"value": "-3.539998272044692E-11", "module": "D", "scenario": "Recycling"}, {"name": "referenceToUnitGroupDataSet", "value": {"shortDescription": [{"value": "kg CFC-11-eq.", "lang": "en"}], "type": "unit group data set", "refObjectId": "d9e957c9-7309-4474-bf3a-7777df6c4e5b", "version": "25.00.000", "uri": "../unitgroups/d9e957c9-7309-4474-bf3a-7777df6c4e5b.xml"}}]}}, {"referenceToLCIAMethodDataSet": {"shortDescription": [{"value": "Acidification potential, Accumulated Exceedance (AP)", "lang": "en"}, {"value": "Versauerungspotenzial, kumulierte Überschreitung (AP)", "lang": "de"}], "type": "LCIA method data set", "refObjectId": "b5c611c6-def3-11e6-bf01-fe55135034f3", "version": "01.03.010", "uri": "../lciamethods/b5c611c6-def3-11e6-bf01-fe55135034f3.xml"}, "meanAmount": 0.0, "other": {"anies": [{"value": "1.08527441441229", "module": "A1-A3"}, {"value": "0.00304119012750499", "module": "A4"}, {"value": "0.0559680689009675", "module": "A5"}, {"value": "0.0", "module": "B1"}, {"value": "0.0", "module": "B2"}, {"value": "0.0", "module": "B3"}, {"value": "0.0", "module": "B4"}, {"value": "0.0", "module": "B5"}, {"value": "0.0", "module": "B6"}, {"value": "0.0", "module": "B7"}, {"value": "0.0", "module": "C1", "scenario": "Energierückgewinnung"}, {"value": "0.00137549807326859", "module": "C2", "scenario": "Energierückgewinnung"}, {"value": "0.0288342763093379", "module": "C3", "scenario": "Energierückgewinnung"}, {"value": "0.0", "module": "C4", "scenario": "Energierückgewinnung"}, {"value": "-0.052090697384290736", "module": "D", "scenario": "Energierückgewinnung"}, {"value": "0.0", "module": "C1", "scenario": "Recycling"}, {"value": "0.00137549807326859", "module": "C2", "scenario": "Recycling"}, {"value": "0.0228653622777134", "module": "C3", "scenario": "Recycling"}, {"value": "0.0", "module": "C4", "scenario": "Recycling"}, {"value": "-0.008022409929616971", "module": "D", "scenario": "Recycling"}, {"name": "referenceToUnitGroupDataSet", "value": {"shortDescription": [{"value": "mol H+-eq.", "lang": "en"}], "type": "unit group data set", "refObjectId": "42e089ac-92bf-4bf2-8ca1-5fc40d18f2ed", "version": "00.01.000", "uri": "../unitgroups/42e089ac-92bf-4bf2-8ca1-5fc40d18f2ed.xml"}}]}}, {"referenceToLCIAMethodDataSet": {"shortDescription": [{"value": "Eutrophication potential - freshwater (EP-freshwater)", "lang": "en"}, {"value": "Eutrophierungspotenzial - Süßwasser (EP-freshwater)", "lang": "de"}], "type": "LCIA method data set", "refObjectId": "b53ec18f-7377-4ad3-86eb-cc3f4f276b2b", "version": "01.00.011", "uri": "../lciamethods/b53ec18f-7377-4ad3-86eb-cc3f4f276b2b.xml"}, "meanAmount": 0.0, "other": {"anies": [{"value": "0.00237840547151944", "module": "A1-A3"}, {"value": "5.59301599194453E-6", "module": "A4"}, {"value": "1.19623462462394E-4", "module": "A5"}, {"value": "0.0", "module": "B1"}, {"value": "0.0", "module": "B2"}, {"value": "0.0", "module": "B3"}, {"value": "0.0", "module": "B4"}, {"value": "0.0", "module": "B5"}, {"value": "0.0", "module": "B6"}, {"value": "0.0", "module": "B7"}, {"value": "0.0", "module": "C1", "scenario": "Energierückgewinnung"}, {"value": "2.68807335264995E-6", "module": "C2", "scenario": "Energierückgewinnung"}, {"value": "5.62763135510322E-6", "module": "C3", "scenario": "Energierückgewinnung"}, {"value": "0.0", "module": "C4", "scenario": "Energierückgewinnung"}, {"value": "-1.4101634172928955E-4", "module": "D", "scenario": "Energierückgewinnung"}, {"value": "0.0", "module": "C1", "scenario": "Recycling"}, {"value": "2.68807335264995E-6", "module": "C2", "scenario": "Recycling"}, {"value": "1.06055002316724E-5", "module": "C3", "scenario": "Recycling"}, {"value": "0.0", "module": "C4", "scenario": "Recycling"}, {"value": "-8.98891469768827E-6", "module": "D", "scenario": "Recycling"}, {"name": "referenceToUnitGroupDataSet", "value": {"shortDescription": [{"value": "kg P-eq.", "lang": "en"}], "type": "unit group data set", "refObjectId": "0429039d-a61d-4590-ba67-aa4a20a810a1", "version": "30.00.000", "uri": "../unitgroups/0429039d-a61d-4590-ba67-aa4a20a810a1.xml"}}]}}, {"referenceToLCIAMethodDataSet": {"shortDescription": [{"value": "Eutrophication potential - marine (EP-marine)", "lang": "en"}, {"value": "Eutrophierungspotenzial - Salzwasser (EP-marine)", "lang": "de"}], "type": "LCIA method data set", "refObjectId": "b5c619fa-def3-11e6-bf01-fe55135034f3", "version": "02.00.011", "uri": "../lciamethods/b5c619fa-def3-11e6-bf01-fe55135034f3.xml"}, "meanAmount": 0.0, "other": {"anies": [{"value": "0.22523753722856", "module": "A1-A3"}, {"value": "0.00114620950130115", "module": "A4"}, {"value": "0.0117530073530095", "module": "A5"}, {"value": "0.0", "module": "B1"}, {"value": "0.0", "module": "B2"}, {"value": "0.0", "module": "B3"}, {"value": "0.0", "module": "B4"}, {"value": "0.0", "module": "B5"}, {"value": "0.0", "module": "B6"}, {"value": "0.0", "module": "B7"}, {"value": "0.0", "module": "C1", "scenario": "Energierückgewinnung"}, {"value": "5.0835411969408E-4", "module": "C2", "scenario": "Energierückgewinnung"}, {"value": "0.00803079448127131", "module": "C3", "scenario": "Energierückgewinnung"}, {"value": "0.0", "module": "C4", "scenario": "Energierückgewinnung"}, {"value": "-0.018823117675393273", "module": "D", "scenario": "Energierückgewinnung"}, {"value": "0.0", "module": "C1", "scenario": "Recycling"}, {"value": "5.0835411969408E-4", "module": "C2", "scenario": "Recycling"}, {"value": "0.00828555379743619", "module": "C3", "scenario": "Recycling"}, {"value": "0.0", "module": "C4", "scenario": "Recycling"}, {"value": "-0.003161205159495672", "module": "D", "scenario": "Recycling"}, {"name": "referenceToUnitGroupDataSet", "value": {"shortDescription": [{"value": "kg N-eq.", "lang": "en"}], "type": "unit group data set", "refObjectId": "d05bb823-ecdf-4686-8c40-bf1d9257859f", "version": "00.00.003", "uri": "../unitgroups/d05bb823-ecdf-4686-8c40-bf1d9257859f.xml"}}]}}, {"referenceToLCIAMethodDataSet": {"shortDescription": [{"value": "Eutrophication potential - terrestrial (EP-terrestrial)", "lang": "en"}, {"value": "Eutrophierungspotenzial - Land (EP-terrestrial)", "lang": "de"}], "type": "LCIA method data set", "refObjectId": "b5c614d2-def3-11e6-bf01-fe55135034f3", "version": "01.02.010", "uri": "../lciamethods/b5c614d2-def3-11e6-bf01-fe55135034f3.xml"}, "meanAmount": 0.0, "other": {"anies": [{"value": "4.97902547669127", "module": "A1-A3"}, {"value": "0.0137738902059707", "module": "A4"}, {"value": "0.257057767692924", "module": "A5"}, {"value": "0.0", "module": "B1"}, {"value": "0.0", "module": "B2"}, {"value": "0.0", "module": "B3"}, {"value": "0.0", "module": "B4"}, {"value": "0.0", "module": "B5"}, {"value": "0.0", "module": "B6"}, {"value": "0.0", "module": "B7"}, {"value": "0.0", "module": "C1", "scenario": "Energierückgewinnung"}, {"value": "0.00613117430449647", "module": "C2", "scenario": "Energierückgewinnung"}, {"value": "0.138326240629002", "module": "C3", "scenario": "Energierückgewinnung"}, {"value": "0.0", "module": "C4", "scenario": "Energierückgewinnung"}, {"value": "-0.19997330107120356", "module": "D", "scenario": "Energierückgewinnung"}, {"value": "0.0", "module": "C1", "scenario": "Recycling"}, {"value": "0.00613117430449647", "module": "C2", "scenario": "Recycling"}, {"value": "0.0906346479932317", "module": "C3", "scenario": "Recycling"}, {"value": "0.0", "module": "C4", "scenario": "Recycling"}, {"value": "-0.03418353212829416", "module": "D", "scenario": "Recycling"}, {"name": "referenceToUnitGroupDataSet", "value": {"shortDescription": [{"value": "mol N-eq.", "lang": "en"}], "type": "unit group data set", "refObjectId": "71b4d617-0ec9-4d3f-b65e-e438940c2401", "version": "00.00.003", "uri": "../unitgroups/71b4d617-0ec9-4d3f-b65e-e438940c2401.xml"}}]}}, {"referenceToLCIAMethodDataSet": {"shortDescription": [{"value": "Photochemical Ozone Creation Potential (POCP)", "lang": "en"}, {"value": "Bildungspotenzial für troposphärisches Ozon (POCP)", "lang": "de"}], "type": "LCIA method data set", "refObjectId": "b5c610fe-def3-11e6-bf01-fe55135034f3", "version": "02.00.015", "uri": "../lciamethods/b5c610fe-def3-11e6-bf01-fe55135034f3.xml"}, "meanAmount": 0.0, "other": {"anies": [{"value": "0.162639830749364", "module": "A1-A3"}, {"value": "0.00298360058591384", "module": "A4"}, {"value": "0.00942399299973315", "module": "A5"}, {"value": "0.0", "module": "B1"}, {"value": "0.0", "module": "B2"}, {"value": "0.0", "module": "B3"}, {"value": "0.0", "module": "B4"}, {"value": "0.0", "module": "B5"}, {"value": "0.0", "module": "B6"}, {"value": "0.0", "module": "B7"}, {"value": "0.0", "module": "C1", "scenario": "Energierückgewinnung"}, {"value": "0.0013527857433855", "module": "C2", "scenario": "Energierückgewinnung"}, {"value": "0.0211304877574106", "module": "C3", "scenario": "Energierückgewinnung"}, {"value": "0.0", "module": "C4", "scenario": "Energierückgewinnung"}, {"value": "-0.049564144308989484", "module": "D", "scenario": "Energierückgewinnung"}, {"value": "0.0", "module": "C1", "scenario": "Recycling"}, {"value": "0.0013527857433855", "module": "C2", "scenario": "Recycling"}, {"value": "0.0243389916799623", "module": "C3", "scenario": "Recycling"}, {"value": "0.0", "module": "C4", "scenario": "Recycling"}, {"value": "-0.01033700437161919", "module": "D", "scenario": "Recycling"}, {"name": "referenceToUnitGroupDataSet", "value": {"shortDescription": [{"value": "kg NMVOC-eq.", "lang": "en"}], "type": "unit group data set", "refObjectId": "d27c25f8-fbc1-44c6-b47b-4adbae4199c6", "version": "00.00.003", "uri": "../unitgroups/d27c25f8-fbc1-44c6-b47b-4adbae4199c6.xml"}}]}}, {"referenceToLCIAMethodDataSet": {"shortDescription": [{"value": "Abiotic depletion potential - non-fossil resources (ADPE)", "lang": "en"}, {"value": "Potenzial für die Verknappung abiotischer Ressourcen – nicht fossile Ressourcen (ADPE)", "lang": "de"}], "type": "LCIA method data set", "refObjectId": "b2ad6494-c78d-11e6-9d9d-cec0c932ce01", "version": "01.00.011", "uri": "../lciamethods/b2ad6494-c78d-11e6-9d9d-cec0c932ce01.xml"}, "meanAmount": 0.0, "other": {"anies": [{"value": "5.28262882828268E-6", "module": "A1-A3"}, {"value": "3.49596136001232E-7", "module": "A4"}, {"value": "3.01071669618453E-7", "module": "A5"}, {"value": "0.0", "module": "B1"}, {"value": "0.0", "module": "B2"}, {"value": "0.0", "module": "B3"}, {"value": "0.0", "module": "B4"}, {"value": "0.0", "module": "B5"}, {"value": "0.0", "module": "B6"}, {"value": "0.0", "module": "B7"}, {"value": "0.0", "module": "C1", "scenario": "Energierückgewinnung"}, {"value": "1.68020270052469E-7", "module": "C2", "scenario": "Energierückgewinnung"}, {"value": "2.14141637251821E-7", "module": "C3", "scenario": "Energierückgewinnung"}, {"value": "0.0", "module": "C4", "scenario": "Energierückgewinnung"}, {"value": "-5.39975639706886E-6", "module": "D", "scenario": "Energierückgewinnung"}, {"value": "0.0", "module": "C1", "scenario": "Recycling"}, {"value": "1.68020270052469E-7", "module": "C2", "scenario": "Recycling"}, {"value": "3.59426860169184E-7", "module": "C3", "scenario": "Recycling"}, {"value": "0.0", "module": "C4", "scenario": "Recycling"}, {"value": "-8.4620494276641E-7", "module": "D", "scenario": "Recycling"}, {"name": "referenceToUnitGroupDataSet", "value": {"shortDescription": [{"value": "kg Sb-eq.", "lang": "en"}], "type": "unit group data set", "refObjectId": "54ccd2d9-a32a-4fc2-923d-f2c8c93e89d4", "version": "30.00.000", "uri": "../unitgroups/54ccd2d9-a32a-4fc2-923d-f2c8c93e89d4.xml"}}]}}, {"referenceToLCIAMethodDataSet": {"shortDescription": [{"value": "Abiotic depletion potential - fossil resources (ADPF)", "lang": "en"}, {"value": "Potenzial für die Verknappung abiotischer Ressourcen – fossile Brennstoffe (ADPF)", "lang": "de"}], "type": "LCIA method data set", "refObjectId": "b2ad6110-c78d-11e6-9d9d-cec0c932ce01", "version": "01.00.011", "uri": "../lciamethods/b2ad6110-c78d-11e6-9d9d-cec0c932ce01.xml"}, "meanAmount": 0.0, "other": {"anies": [{"value": "155.358007479547", "module": "A1-A3"}, {"value": "26.9676389812159", "module": "A4"}, {"value": "11.4308960619465", "module": "A5"}, {"value": "0.0", "module": "B1"}, {"value": "0.0", "module": "B2"}, {"value": "0.0", "module": "B3"}, {"value": "0.0", "module": "B4"}, {"value": "0.0", "module": "B5"}, {"value": "0.0", "module": "B6"}, {"value": "0.0", "module": "B7"}, {"value": "0.0", "module": "C1", "scenario": "Energierückgewinnung"}, {"value": "12.9609841691311", "module": "C2", "scenario": "Energierückgewinnung"}, {"value": "35.8198172411363", "module": "C3", "scenario": "Energierückgewinnung"}, {"value": "0.0", "module": "C4", "scenario": "Energierückgewinnung"}, {"value": "-819.456981073288", "module": "D", "scenario": "Energierückgewinnung"}, {"value": "0.0", "module": "C1", "scenario": "Recycling"}, {"value": "12.9609841691311", "module": "C2", "scenario": "Recycling"}, {"value": "24.347930453478", "module": "C3", "scenario": "Recycling"}, {"value": "0.0", "module": "C4", "scenario": "Recycling"}, {"value": "-441.423176405349", "module": "D", "scenario": "Recycling"}, {"name": "referenceToUnitGroupDataSet", "value": {"shortDescription": [{"value": "MJ", "lang": "en"}], "type": "unit group data set", "refObjectId": "93a60a57-a3c8-11da-a746-0800200c9a66", "version": "03.00.000", "uri": "../unitgroups/93a60a57-a3c8-11da-a746-0800200c9a66.xml"}}]}}, {"referenceToLCIAMethodDataSet": {"shortDescription": [{"value": "Water (user) deprivation potential (WDP)", "lang": "en"}, {"value": "Wasser-Entzugspotenzial (Benutzer) (WDP)", "lang": "de"}], "type": "LCIA method data set", "refObjectId": "b2ad66ce-c78d-11e6-9d9d-cec0c932ce01", "version": "03.00.015", "uri": "../lciamethods/b2ad66ce-c78d-11e6-9d9d-cec0c932ce01.xml"}, "meanAmount": 0.0, "other": {"anies": [{"value": "0.712659741911093", "module": "A1-A3"}, {"value": "0.0147209487033844", "module": "A4"}, {"value": "0.883154395486355", "module": "A5"}, {"value": "0.0", "module": "B1"}, {"value": "0.0", "module": "B2"}, {"value": "0.0", "module": "B3"}, {"value": "0.0", "module": "B4"}, {"value": "0.0", "module": "B5"}, {"value": "0.0", "module": "B6"}, {"value": "0.0", "module": "B7"}, {"value": "0.0", "module": "C1", "scenario": "Energierückgewinnung"}, {"value": "0.00707507183821532", "module": "C2", "scenario": "Energierückgewinnung"}, {"value": "16.4390126115631", "module": "C3", "scenario": "Energierückgewinnung"}, {"value": "0.0", "module": "C4", "scenario": "Energierückgewinnung"}, {"value": "-0.7416505826926959", "module": "D", "scenario": "Energierückgewinnung"}, {"value": "0.0", "module": "C1", "scenario": "Recycling"}, {"value": "0.00707507183821532", "module": "C2", "scenario": "Recycling"}, {"value": "0.219631005205569", "module": "C3", "scenario": "Recycling"}, {"value": "0.0", "module": "C4", "scenario": "Recycling"}, {"value": "-0.0555997967130417", "module": "D", "scenario": "Recycling"}, {"name": "referenceToUnitGroupDataSet", "value": {"shortDescription": [{"value": "m3 world eq. deprived", "lang": "en"}], "type": "unit group data set", "refObjectId": "6ae2df01-888e-46c8-b17d-49fa3869b476", "version": "00.00.003", "uri": "../unitgroups/6ae2df01-888e-46c8-b17d-49fa3869b476.xml"}}]}}, {"referenceToLCIAMethodDataSet": {"shortDescription": [{"value": "Potential incidence of disease due to PM emissions (PM)", "lang": "en"}, {"value": "Potenzielles Auftreten von Krankheiten aufgrund von Feinstaubemissionen (PM)", "lang": "de"}], "type": "LCIA method data set", "refObjectId": "b5c602c6-def3-11e6-bf01-fe55135034f3", "version": "02.00.012", "uri": "../lciamethods/b5c602c6-def3-11e6-bf01-fe55135034f3.xml"}, "meanAmount": 0.0, "other": {"anies": [{"value": "7.81802536845308E-6", "module": "A1-A3"}, {"value": "2.77831968403711E-8", "module": "A4"}, {"value": "4.0085269644048E-7", "module": "A5"}, {"value": "0.0", "module": "B1"}, {"value": "0.0", "module": "B2"}, {"value": "0.0", "module": "B3"}, {"value": "0.0", "module": "B4"}, {"value": "0.0", "module": "B5"}, {"value": "0.0", "module": "B6"}, {"value": "0.0", "module": "B7"}, {"value": "0.0", "module": "C1", "scenario": "Energierückgewinnung"}, {"value": "1.28169715143287E-8", "module": "C2", "scenario": "Energierückgewinnung"}, {"value": "1.53115378270297E-7", "module": "C3", "scenario": "Energierückgewinnung"}, {"value": "0.0", "module": "C4", "scenario": "Energierückgewinnung"}, {"value": "-3.6843154030058764E-7", "module": "D", "scenario": "Energierückgewinnung"}, {"value": "0.0", "module": "C1", "scenario": "Recycling"}, {"value": "1.28169715143287E-8", "module": "C2", "scenario": "Recycling"}, {"value": "1.48771201870223E-7", "module": "C3", "scenario": "Recycling"}, {"value": "0.0", "module": "C4", "scenario": "Recycling"}, {"value": "-6.46430371048681E-8", "module": "D", "scenario": "Recycling"}, {"name": "referenceToUnitGroupDataSet", "value": {"shortDescription": [{"value": "Disease incidence", "lang": "en"}], "type": "unit group data set", "refObjectId": "3883559b-648f-4afc-8ba2-0bd24f3affa3", "version": "00.00.003", "uri": "../unitgroups/3883559b-648f-4afc-8ba2-0bd24f3affa3.xml"}}]}}, {"referenceToLCIAMethodDataSet": {"shortDescription": [{"value": "Potential Human exposure efficiency relative to U235 (IRP)", "lang": "en"}, {"value": "Potenzielle Wirkung durch Exposition des Menschen mit U235 (IRP)", "lang": "de"}], "type": "LCIA method data set", "refObjectId": "b5c632be-def3-11e6-bf01-fe55135034f3", "version": "01.00.012", "uri": "../lciamethods/b5c632be-def3-11e6-bf01-fe55135034f3.xml"}, "meanAmount": 0.0, "other": {"anies": [{"value": "0.211887958295316", "module": "A1-A3"}, {"value": "0.00452825750179343", "module": "A4"}, {"value": "0.0168762667679404", "module": "A5"}, {"value": "0.0", "module": "B1"}, {"value": "0.0", "module": "B2"}, {"value": "0.0", "module": "B3"}, {"value": "0.0", "module": "B4"}, {"value": "0.0", "module": "B5"}, {"value": "0.0", "module": "B6"}, {"value": "0.0", "module": "B7"}, {"value": "0.0", "module": "C1", "scenario": "Energierückgewinnung"}, {"value": "0.00217633712151718", "module": "C2", "scenario": "Energierückgewinnung"}, {"value": "0.116634340987608", "module": "C3", "scenario": "Energierückgewinnung"}, {"value": "0.0", "module": "C4", "scenario": "Energierückgewinnung"}, {"value": "-3.174792392015351", "module": "D", "scenario": "Energierückgewinnung"}, {"value": "0.0", "module": "C1", "scenario": "Recycling"}, {"value": "0.00217633712151718", "module": "C2", "scenario": "Recycling"}, {"value": "0.238850026351424", "module": "C3", "scenario": "Recycling"}, {"value": "0.0", "module": "C4", "scenario": "Recycling"}, {"value": "-0.16497423959793553", "module": "D", "scenario": "Recycling"}, {"name": "referenceToUnitGroupDataSet", "value": {"shortDescription": [{"value": "kgBq U235-eq.", "lang": "en"}], "type": "unit group data set", "refObjectId": "456b05bf-1415-44a9-9993-02452f554c09", "version": "00.00.003", "uri": "../unitgroups/456b05bf-1415-44a9-9993-02452f554c09.xml"}}]}}, {"referenceToLCIAMethodDataSet": {"shortDescription": [{"value": "Potential Comparative Toxic Unit for ecosystems (ETP-fw)", "lang": "en"}, {"value": "Potenzielle Toxizitätsvergleichseinheit für Ökosysteme (ETP-fw)", "lang": "de"}], "type": "LCIA method data set", "refObjectId": "05316e7a-b254-4bea-9cf0-6bf33eb5c630", "version": "01.00.003", "uri": "../lciamethods/05316e7a-b254-4bea-9cf0-6bf33eb5c630.xml"}, "meanAmount": 0.0, "other": {"anies": [{"value": "94.8447525356484", "module": "A1-A3"}, {"value": "20.9295508391043", "module": "A4"}, {"value": "7.0211587025123", "module": "A5"}, {"value": "0.0", "module": "B1"}, {"value": "0.0", "module": "B2"}, {"value": "0.0", "module": "B3"}, {"value": "0.0", "module": "B4"}, {"value": "0.0", "module": "B5"}, {"value": "0.0", "module": "B6"}, {"value": "0.0", "module": "B7"}, {"value": "0.0", "module": "C1", "scenario": "Energierückgewinnung"}, {"value": "10.0587465962555", "module": "C2", "scenario": "Energierückgewinnung"}, {"value": "14.1221806317805", "module": "C3", "scenario": "Energierückgewinnung"}, {"value": "0.0", "module": "C4", "scenario": "Energierückgewinnung"}, {"value": "-121.7358366933343", "module": "D", "scenario": "Energierückgewinnung"}, {"value": "0.0", "module": "C1", "scenario": "Recycling"}, {"value": "10.0587465962555", "module": "C2", "scenario": "Recycling"}, {"value": "9.41273545631129", "module": "C3", "scenario": "Recycling"}, {"value": "0.0", "module": "C4", "scenario": "Recycling"}, {"value": "-11.15792507560781", "module": "D", "scenario": "Recycling"}, {"name": "referenceToUnitGroupDataSet", "value": {"shortDescription": [{"value": "CTUe", "lang": "en"}], "type": "unit group data set", "refObjectId": "aa959ded-f1eb-4efb-9c5c-2d60be36b3e6", "version": "00.00.003", "uri": "../unitgroups/aa959ded-f1eb-4efb-9c5c-2d60be36b3e6.xml"}}]}}, {"referenceToLCIAMethodDataSet": {"shortDescription": [{"value": "Potential Comparative Toxic Unit for humans - cancer effects (HTP-c)", "lang": "en"}, {"value": "Potenzielle Toxizitätsvergleichseinheit für den Menschen - kanzerogene Wirkung (HTP-c)", "lang": "de"}], "type": "LCIA method data set", "refObjectId": "2299222a-bbd8-474f-9d4f-4dd1f18aea7c", "version": "01.00.004", "uri": "../lciamethods/2299222a-bbd8-474f-9d4f-4dd1f18aea7c.xml"}, "meanAmount": 0.0, "other": {"anies": [{"value": "1.3441681761091E-7", "module": "A1-A3"}, {"value": "4.17265289146739E-10", "module": "A4"}, {"value": "6.80651481988161E-9", "module": "A5"}, {"value": "0.0", "module": "B1"}, {"value": "0.0", "module": "B2"}, {"value": "0.0", "module": "B3"}, {"value": "0.0", "module": "B4"}, {"value": "0.0", "module": "B5"}, {"value": "0.0", "module": "B6"}, {"value": "0.0", "module": "B7"}, {"value": "0.0", "module": "C1", "scenario": "Energierückgewinnung"}, {"value": "2.00536939285258E-10", "module": "C2", "scenario": "Energierückgewinnung"}, {"value": "1.05682050254525E-9", "module": "C3", "scenario": "Energierückgewinnung"}, {"value": "0.0", "module": "C4", "scenario": "Energierückgewinnung"}, {"value": "-8.789525173066555E-9", "module": "D", "scenario": "Energierückgewinnung"}, {"value": "0.0", "module": "C1", "scenario": "Recycling"}, {"value": "2.00536939285258E-10", "module": "C2", "scenario": "Recycling"}, {"value": "5.27441738235697E-9", "module": "C3", "scenario": "Recycling"}, {"value": "0.0", "module": "C4", "scenario": "Recycling"}, {"value": "-2.148662371767285E-9", "module": "D", "scenario": "Recycling"}, {"name": "referenceToUnitGroupDataSet", "value": {"shortDescription": [{"value": "CTUh", "lang": "en"}], "type": "unit group data set", "refObjectId": "d4c9523e-2d7e-49fd-8469-998f547d3a70", "version": "00.00.003", "uri": "../unitgroups/d4c9523e-2d7e-49fd-8469-998f547d3a70.xml"}}]}}, {"referenceToLCIAMethodDataSet": {"shortDescription": [{"value": "Potential Comparative Toxic Unit for humans - non-cancer effects (HTP-nc)", "lang": "en"}, {"value": "Potenzielle Toxizitätsvergleichseinheit für den Menschen - nicht kanzerogene Wirkung (HTP-nc)", "lang": "de"}], "type": "LCIA method data set", "refObjectId": "7cfdcfcf-b222-4b26-888a-a55f9fbf7ac8", "version": "01.00.003", "uri": "../lciamethods/7cfdcfcf-b222-4b26-888a-a55f9fbf7ac8.xml"}, "meanAmount": 0.0, "other": {"anies": [{"value": "1.61509373324301E-5", "module": "A1-A3"}, {"value": "1.75776560354953E-8", "module": "A4"}, {"value": "8.09632219248148E-7", "module": "A5"}, {"value": "0.0", "module": "B1"}, {"value": "0.0", "module": "B2"}, {"value": "0.0", "module": "B3"}, {"value": "0.0", "module": "B4"}, {"value": "0.0", "module": "B5"}, {"value": "0.0", "module": "B6"}, {"value": "0.0", "module": "B7"}, {"value": "0.0", "module": "C1", "scenario": "Energierückgewinnung"}, {"value": "8.44784162919743E-9", "module": "C2", "scenario": "Energierückgewinnung"}, {"value": "1.52424597362984E-8", "module": "C3", "scenario": "Energierückgewinnung"}, {"value": "0.0", "module": "C4", "scenario": "Energierückgewinnung"}, {"value": "-3.1649562458755003E-7", "module": "D", "scenario": "Energierückgewinnung"}, {"value": "0.0", "module": "C1", "scenario": "Recycling"}, {"value": "8.44784162919743E-9", "module": "C2", "scenario": "Recycling"}, {"value": "2.74303865685639E-8", "module": "C3", "scenario": "Recycling"}, {"value": "0.0", "module": "C4", "scenario": "Recycling"}, {"value": "-1.93127541014063E-7", "module": "D", "scenario": "Recycling"}, {"name": "referenceToUnitGroupDataSet", "value": {"shortDescription": [{"value": "CTUh", "lang": "en"}], "type": "unit group data set", "refObjectId": "d4c9523e-2d7e-49fd-8469-998f547d3a70", "version": "00.00.003", "uri": "../unitgroups/d4c9523e-2d7e-49fd-8469-998f547d3a70.xml"}}]}}, {"referenceToLCIAMethodDataSet": {"shortDescription": [{"value": "Potential Soil quality index (SQP)", "lang": "en"}, {"value": "Potenzieller Bodenqualitätsindex (SQP)", "lang": "de"}], "type": "LCIA method data set", "refObjectId": "b2ad6890-c78d-11e6-9d9d-cec0c932ce01", "version": "01.00.011", "uri": "../lciamethods/b2ad6890-c78d-11e6-9d9d-cec0c932ce01.xml"}, "meanAmount": 0.0, "other": {"anies": [{"value": "6674.38823902983", "module": "A1-A3"}, {"value": "17.9400170614299", "module": "A4"}, {"value": "335.697137133611", "module": "A5"}, {"value": "0.0", "module": "B1"}, {"value": "0.0", "module": "B2"}, {"value": "0.0", "module": "B3"}, {"value": "0.0", "module": "B4"}, {"value": "0.0", "module": "B5"}, {"value": "0.0", "module": "B6"}, {"value": "0.0", "module": "B7"}, {"value": "0.0", "module": "C1", "scenario": "Energierückgewinnung"}, {"value": "8.6221963030985", "module": "C2", "scenario": "Energierückgewinnung"}, {"value": "12.6014854997407", "module": "C3", "scenario": "Energierückgewinnung"}, {"value": "0.0", "module": "C4", "scenario": "Energierückgewinnung"}, {"value": "-218.5884841578605", "module": "D", "scenario": "Energierückgewinnung"}, {"value": "0.0", "module": "C1", "scenario": "Recycling"}, {"value": "8.6221963030985", "module": "C2", "scenario": "Recycling"}, {"value": "16.7405382714317", "module": "C3", "scenario": "Recycling"}, {"value": "0.0", "module": "C4", "scenario": "Recycling"}, {"value": "-11.855287806093898", "module": "D", "scenario": "Recycling"}, {"name": "referenceToUnitGroupDataSet", "value": {"shortDescription": [{"value": "dimensionless", "lang": "en"}], "type": "unit group data set", "refObjectId": "f130951c-e67f-4f7f-8dd4-665de3974e18", "version": "00.00.004", "uri": "../unitgroups/f130951c-e67f-4f7f-8dd4-665de3974e18.xml"}}]}}]}, "otherAttributes": {"{http://www.indata.network/EPD/2019}epd-version": "1.2", "{http://www.okworx.com/ILCD/Extensions/2018/Profile}profile": "EN_15804"}, "version": "1.1"}