{"processInformation": {"dataSetInformation": {"UUID": "010b169d-881a-47d8-83ea-e74930c4d424", "name": {"baseName": [{"value": "Kunststoff Dach- und Dichtungsbahn Polyfin® 3020", "lang": "de"}, {"value": "Polyfin® 3020 roofing and sealing membranes", "lang": "en"}], "functionalUnitFlowProperties": [{"lang": "de"}]}, "classificationInformation": {"classification": [{"class": [{"value": "Kunststoffe", "level": 0, "classId": "6"}, {"value": "Dachbahnen", "level": 1, "classId": "6.3"}, {"value": "TPO-Dachbahnen (FPO)", "level": 2, "classId": "6.3.05"}], "name": "OEKOBAU.DAT"}, {"class": [{"value": "02 Bauprodukte", "level": 0}, {"value": "Abdichtungen", "level": 1}, {"value": "Dach- und Dichtungsbahnsysteme aus Kunststoffen und Elastomeren", "level": 2}], "name": "IBUCategories"}]}, "generalComment": [{"value": "Polyfin 30.. und Polyfin 40.. v \nDach- und Dichtungsbahnen dieser Produktreihe bestehen aus FPO (flexible Polyolefine). Sie verfgen ber einen mittigen Festigkeitstrger in Form einer Glasvlieseinlage. Bahnen der Polyfin 40.. v-Reihe verfgen zustzlich ber eine unterseitige Kaschierung aus einem Polyestervlies. Die letzten 2 Ziffern in der Produktbezeichnung geben die Dichtschichtdicke in Zehntelmillimetern an: \n\nPolyfin 30.. : \n\nPolyfin 3020 (2,0 mm)\nPolyfin 3018 (1,8 mm) \nPolyfin 3015 (1,5 mm) Polyfin 40.. v: \nPolyfin 4020 v (2,0 mm) \nPolyfin 4018 v (1,8 mm)\nPolyfin 4015 v (1,5 mm) Polyfin Duo 30.. GS und Polyfin Duo 30.. \nDach- und Dichtungsbahnen dieser Produktreihe bestehen aus FPO (flexible Polyolefine). Sie verfgen ber einen mittigen Festigkeitstrger in Form einer Glasvlieseinlage. Bahnen der Polyfin Duo 30.. GS-Reihe verfgen zustzlich zur Glasvlieseinlage ber eine Verstrkung aus einem Polyestergelege. Die letzten 2 Ziffern in der Produktbezeichnung geben die Dichtschichtdicke in Zehntelmillimetern an: \n\nPolyfin Duo 30.. GS: \n\nPolyfin Duo 3020 GS (2,0 mm)\nPolyfin Duo 3018 GS (1,8 mm) \nPolyfin Duo 3015 GS (1,5 mm)Polyfin Duo 30..:\nPolyfin Duo 3020 (2,0 mm)\nPolyfin Duo 3018 (1,8 mm) \nPolyfin Duo 3015 (1,5 mm) Die vorliegende Umwelt-Produktdeklaration bezieht sich auf Polyfin 3020 Dach- und Dichtungsbahnen. \n\nIn einem separaten Annex werden die Umweltwirkungen der folgenden Bahnen ausgewiesen: \nPolyfin 3018, Polyfin 3015 \nPolyfin 4020 v, Polyfin 4018 v, Polyfin 4015 v \nPolyfin Duo 3020 GS, Polyfin Duo 3018 GS, Polyfin Duo 3015 GS\nPolyfin Duo 3020, Polyfin Duo 3018, Polyfin Duo 3015", "lang": "de"}], "other": {"anies": [{"scenario": [{"description": [{"value": "100% stoffliches Recycling", "lang": "de"}], "name": "S1"}, {"description": [{"value": "100% Energierückgewinnung ", "lang": "de"}], "name": "S2", "default": true}]}]}}, "quantitativeReference": {"referenceToReferenceFlow": [0]}, "time": {"referenceYear": 2023, "dataSetValidUntil": 2028, "other": {"anies": [{"name": "publicationDateOfEPD", "value": 1680480000000}]}}, "geography": {"locationOfOperationSupplyOrProduction": {"location": "DE"}}, "technology": {"technologyDescriptionAndIncludedProcesses": [{"value": "Die Herstellung der Dach- und Dichtungsbahnen erfolgt auf einer Zweidüsen Extrusionsanlage. Der Rohstoff wird in den Extrudern auf eine entsprechende Temperatur erwärmt, aufgeschmolzen und unter Druck durch die Breitschlitzdüsen gepresst. Die gewünschte Materialstärke wird über die Öffnung der Extruderdüsen und über ein direkt dahinter befindliches Glättwerk, in welchem auch die unterschiedlichen Lagen des Produktes zusammengeführt werden, erzeugt. Der mittige Festigkeitsträger wird dabei zwischen die beiden extrudierten Kunststofflagen eingebettet. Bei der Polyfin 40.. v Produktreihe wird auf die Unterseite des Produktes noch ein Polyestervlies kaschiert. Nach Verlassen der Kühlstrecke werden die Bahnen auf Rollen gewickelt und auf Paletten versandfertig gestapelt.   Alle während der Produktion anfallenden Bahnenabfälle werden wiederverwendet. So sie nicht direkt wieder zugeführt werden, werden sie fremdvermahlen und als Mahlgut wieder zugeführt.   Das Werk verfügt über ein vom TÜV Süd nach ISO 9001 zertifiziertes Qualitätsmanagementsystem.   Die Qualitätssicherung erfolgt zudem in Übereinstimmung mit den Anforderungen der Normen EN 13956 und EN 13967. \nDeklarierte Einheit: \nDie vorliegende Umwelt-Produktdeklaration bezieht sich auf eine deklarierte Einheit von 1 m Polyfin 3020 Dach- und Dichtungsbahn mit einem Flchengewicht von 2,14 kg/m.", "lang": "de"}, {"value": "The roofing and waterproofing membranes are produced on a two-nozzle extrusion line. The raw material is heated to an appropriate temperature in the extruders, melted and pressed under pressure through the slot dies. The desired material thickness is produced via the opening of the extruder nozzles and via a smoothing unit located directly behind it, in which the different layers of the product are also merged. The central reinforcing is embedded between the two extruded plastic layers. For the Polyfin 40... v product range, a polyester fleece is laminated to the underside of the product. After leaving the cooling line, the membranes are wound onto reels and stacked on pallets ready for shipping. All membrane waste produced during the production process is recycled. If it is not directly fed-back into the production, it is ground by third parties and reintroduced as regrind. The plant has a quality management system certified by TÜV Süd according to ISO 9001. Quality assurance is also carried out in accordance with the requirements of EN 13956 and EN 13967 standards.", "lang": "en"}], "technologicalApplicability": [{"value": "Die Dach- und Dichtungsbahnen werden zur einlagigen Abdichtung von nicht genutzten und genutzten Dchern sowie von nicht wasserdichten Bauwerken und Bauteilen verwendet. \n\nNahtfgetechnik: Die Fgenhte werden auf der Baustelle mittels Heiluftschweiung hergestellt. \n\nLagesicherung: Die Bahnen werden mechanisch befestigt oder lose verlegt und mittels Auflast in der Lage gesichert. Bahnen der Polyfin 40.. v-Reihe knnen darber hinaus mit geeigneten Klebern zum Untergrund verklebt werden.", "lang": "de"}, {"value": "The roofing and waterproofing membranes are used for single-ply waterproofing of unused and used roofs as well as non-waterproof structures and building components. Seam joining technology: The joining seams are produced on site by means of hot air welding. Position securing: The membranes are mechanically fastened or loosely laid and secured in position by means of ballast. Polyfin 40... v sheets can also be bonded to the substrate with suitable adhesives.", "lang": "en"}]}}, "modellingAndValidation": {"LCIMethodAndAllocation": {"typeOfDataSet": "EPD", "referenceToLCAMethodDetails": [{"shortDescription": [{"value": "Dach- und Dichtungsbahnsysteme aus Kunststoffen und Elastomeren.pdf", "lang": "de"}], "type": "source data set", "refObjectId": "dd8270f8-c8c6-4494-9285-189857ae12b4"}], "other": {"anies": [{"name": "subType", "value": "specific dataset"}]}}, "dataSourcesTreatmentAndRepresentativeness": {"referenceToDataSource": [{"shortDescription": [{"value": "GaBi Database (all versions)", "lang": "de"}], "type": "source data set", "refObjectId": "28d74cc0-db8b-4d7e-bc44-5f6d56ce0c4a"}, {"shortDescription": [{"value": "GaBi Database Edition 2022, CUP 2022.02", "lang": "de"}], "type": "source data set", "refObjectId": "94f442cb-662e-43ea-a792-4b0a35132e93"}], "useAdviceForDataSet": [{"value": "Gültigkeitsbereich: \nDie vorliegende Umwelt-Produktdeklaration bezieht sich auf eine deklarierte Einheit von 1 m Polyfin 3020 Dach- und Dichtungsbahn aus FPO mit einem Flchengewicht von 2,14 kg/m, produziert am Standort Meckesheim (Deutschland).\nEin separater Annex enthlt die Ergebnisse fr die folgenden am Standort Meckesheim hergestellten Dach- und Dichtungsbahnen aus FPO:\n\nPolyfin 3018, Polyfin 3015\nPolyfin 4020 v, Polyfin 4018 v, Polyfin 4015 v\nPolyfin Duo 3020 GS, Polyfin Duo 3018 GS, Polyfin Duo 3015 GS\nPolyfin Duo 3020, Polyfin Duo 3018, Polyfin Duo 3015 \nSystemgrenze: \nDie kobilanz der Polyfin-Dachbahnen beinhaltet eine cradle-to-gate (Wiege bis zum Werkstor)-Betrachtung mit den Modulen C1–C4 und Modul D (A1–A3, +C, +D). Die folgenden Lebenszyklusphasen werden in der Analyse bercksichtigt:\n\nModul A1–A3 | Produktionsstadium\nDas Produktionsstadium beinhaltet die Aufwendungen der Herstellung der eingesetzten Grundstoffe (FPO/PE, Glasvlies etc.) sowie der damit verbundenen Transporte der Rohstoffe. Die Abbildung der Produktion der Dachbahnen innerhalb der Werksgrenzen in Meckesheim bercksichtigt alle Prozessschritte am Standort (Extrusion etc.). Die thermische Energiebereitstellung am Standort erfolgt ber Erdgas, elektrische Energie wird vom regionalen Stromnetz bezogen. Auch die Produktion der zur Auslieferung der Produkte eingesetzten Verpackung ist in Modul A1–A3 erfasst.\n\nModul C1 | Rckbau\nFr die Dachbahnen wurde ein manueller Ausbau angenommen. Der sortenreine Rckbau der Produkte ist blicherweise mglich. Die damit verbundenen Aufwnde sind vernachlssigbar, wodurch keine Umweltwirkungen aus dem Rckbau der Produkte deklariert werden.\nModul C2/1 | Transport zum stofflichen Recycling\nModul C2 beinhaltet den Transport zur Abfallbehandlung. Fr Szenario 1 wird der Transport zum stofflichen Recycling via LKW ber 300 km Transportdistanz angesetzt.\n\nModul C2/2 | Transport zur Energierckgewinnung\nIn Szenario 2, der energetischen Verwertung der Produkte, wird der Transport via LKW ber 50 km Transportdistanz angesetzt.\nModul C3/1 | Abfallbehandlung beim stofflichen Recycling\nIn Szenario 1 beinhaltet das Modul C3 die Zerkleinerung der Dachbahnen als Ausgangsmaterial fr das anschlieende stoffliche Recycling. Jener Produktfluss, der das Modul D zum Recycling erreicht, verlsst das Produktsystem in C3.\nModul C3/2 | Abfallbehandlung bei der Energierckgewinnung\nDas Szenario 2 sieht eine energetische Verwertung der Dachbahnen nach Ausbau aus dem Gebude von 100 % vor. Es wird angenommen, dass die Dachbahnen am Lebensende in einer Mllverbrennungsanlage zur Erzeugung von Energie verwertet werden. Die Emissionen aus der Verbrennung sind dabei in Modul C3 deklariert. Basierend auf Informationen von Sphera (siehe GaBi) wird ein R1-Wert der Mllverbrennungsanlage von > 0,6 angenommen.\n\nModul C4/1 | Entsorgung beim stofflichen Recycling\nDas angesetzte Szenario 1 deklariert die stoffliche Verwertung der Dachbahnen, wodurch keine Umweltauswirkungen aus der Entsorgung der Produkte in C4 zu erwarten sind.\nModul C4/2 | Abfallbeseitigung bei der Energierckgewinnung\nDie Umweltlasten aus der energetischen Verwertung (Szenario 2) der deklarierten Produkte werden in Modul C3 deklariert. Somit sind keine Aufwnde in Modul C4 zu deklarieren.\n\nModul D/1 | Gutschriften und Lasten auerhalb der Systemgrenzen beim Recycling\nIm Modul D/1 wird ein Recyclingszenario unter Bercksichtigung der Substitutionspotenziale von fossilem Polyethylen-Primrmaterial deklariert.\n\nModul D/2 | Gutschriften und Lasten auerhalb der Systemgrenzen bei der Energierckgewinnung\nModul D/2 deklariert die Substitutionspotenziale fr Wrme und Strom aus der energetischen Verwertung des Produktes in Modul C3 in Form eines europischen Durchschnittsszenarios.", "lang": "de"}], "other": {"anies": [{"name": "referenceToOriginalEPD", "value": {"shortDescription": {"value": "Kunststoff Dach- und Dichtungsbahn Polyfin® 3020.pdf", "defaultValue": "Kunststoff Dach- und Dichtungsbahn Polyfin® 3020.pdf", "lstrings": [{"lang": "de", "value": "Kunststoff Dach- und Dichtungsbahn Polyfin® 3020.pdf"}]}, "type": "source data set", "uuid": {"uuid": "313df8f6-97ed-4d15-bb08-909c2c5302fd"}, "refObjectId": "313df8f6-97ed-4d15-bb08-909c2c5302fd", "resourceURLs": ["https://oekobaudat.de/OEKOBAU.DAT/resource/sources/313df8f6-97ed-4d15-bb08-909c2c5302fd/Kunststoff_Dach-_und_Dichtungsbahn_Polyfin_3020_18534.pdf?version=00.02.000"]}}]}}, "validation": {"review": [{"referenceToNameOfReviewerAndInstitution": [{"shortDescription": [{"value": "Institut Bauen und Umwelt e. V.", "lang": "de"}], "type": "contact data set", "refObjectId": "d111dbec-b024-4be5-86c5-752d6eb2cf95", "uri": "../contacts/d111dbec-b024-4be5-86c5-752d6eb2cf95.xml"}], "type": "Accredited third party review"}]}, "complianceDeclarations": {"compliance": [{"referenceToComplianceSystem": {"shortDescription": [{"value": "DIN EN 15804+A2", "lang": "de"}], "type": "source data set", "refObjectId": "c0016b33-8cf7-415c-ac6e-deba0d21440d", "uri": "../sources/c0016b33-8cf7-415c-ac6e-deba0d21440d.xml"}}, {"referenceToComplianceSystem": {"shortDescription": [{"value": "ISO 14025", "lang": "de"}], "type": "source data set", "refObjectId": "4f2eb655-6e44-4874-a95a-e28f5442cd4d", "uri": "../sources/4f2eb655-6e44-4874-a95a-e28f5442cd4d.xml"}}]}}, "administrativeInformation": {"commissionerAndGoal": {"referenceToCommissioner": [{"shortDescription": [{"value": "POLYFIN AG", "lang": "de"}], "type": "contact data set", "refObjectId": "39dab5d3-ea20-4cb7-8298-404d5c85dd66", "uri": "../contacts/39dab5d3-ea20-4cb7-8298-404d5c85dd66.xml"}]}, "dataGenerator": {"referenceToPersonOrEntityGeneratingTheDataSet": [{"shortDescription": [{"value": "Daxner & Merl GmbH", "lang": "de"}], "type": "contact data set", "refObjectId": "ad8ad627-3991-42b7-a7ca-5a3fe0a34c28", "uri": "../contacts/ad8ad627-3991-42b7-a7ca-5a3fe0a34c28.xml"}]}, "dataEntryBy": {"timeStamp": 1680480000000, "referenceToDataSetFormat": [{"shortDescription": [{"value": "ILCD Format", "lang": "de"}], "type": "source data set", "refObjectId": "a97a0155-0234-4b87-b4ce-a45da52f2a40", "uri": "../sources/a97a0155-0234-4b87-b4ce-a45da52f2a40.xml"}, {"shortDescription": [{"value": "EPD-Datenformaterweiterungen v1.2", "lang": "de"}, {"value": "EPD Data Format Extensions v1.2", "lang": "en"}], "type": "source data set", "refObjectId": "a29449fd-aa2f-4de8-b5d7-4b06b43c6fde", "uri": "../sources/a29449fd-aa2f-4de8-b5d7-4b06b43c6fde.xml"}]}, "publicationAndOwnership": {"dataSetVersion": "00.07.000", "referenceToRegistrationAuthority": {"shortDescription": [{"value": "Institut Bauen und Umwelt e. V.", "lang": "de"}], "type": "contact data set", "refObjectId": "d111dbec-b024-4be5-86c5-752d6eb2cf95", "uri": "../contacts/d111dbec-b024-4be5-86c5-752d6eb2cf95.xml"}, "registrationNumber": "EPD-POL-20230126-IBA1-DE", "referenceToOwnershipOfDataSet": {"shortDescription": [{"value": "POLYFIN AG", "lang": "de"}], "type": "contact data set", "refObjectId": "39dab5d3-ea20-4cb7-8298-404d5c85dd66", "uri": "../contacts/39dab5d3-ea20-4cb7-8298-404d5c85dd66.xml"}, "copyright": true, "licenseType": "Free of charge for all users and uses", "accessRestrictions": [{"value": "None", "lang": "en"}], "other": {"anies": [{"name": "referenceToPublisher", "value": {"shortDescription": [{"value": "Institut Bauen und Umwelt e. V.", "lang": "de"}], "type": "contact data set", "refObjectId": "d111dbec-b024-4be5-86c5-752d6eb2cf95", "uri": "../contacts/d111dbec-b024-4be5-86c5-752d6eb2cf95.xml"}}]}}}, "exchanges": {"exchange": [{"dataSetInternalID": 0, "referenceToFlowDataSet": {"shortDescription": [{"value": "Polyfin 3020 Dachbahnen (2,14 kg/m²) (Polyfin 3020 Dachbahnen (2,14 kg/m²))", "lang": "de"}], "type": "flow data set", "refObjectId": "ba26caa1-9d0b-c7cb-d1fc-60e3b1c33b36", "uri": "../flows/ba26caa1-9d0b-c7cb-d1fc-60e3b1c33b36.xml"}, "meanAmount": 1.0, "referencesToDataSource": {}, "referenceFlow": true, "resolvedFlowVersion": "00.02.000", "resultingflowAmount": 1.0, "flowProperties": [{"name": [{"lang": "en", "value": "Area"}, {"lang": "de", "value": "Fläche"}], "uuid": "93a60a56-a3c8-19da-a746-0800200c9a66", "referenceFlowProperty": true, "meanValue": 1.0, "referenceUnit": "qm", "unitGroupUUID": "c20a03d7-bd90-4569-bc94-66cfd364dfc8"}], "materialProperties": [{"name": "layer thickness", "value": "0.002", "unit": "m", "unitDescription": "meters"}, {"name": "grammage", "value": "2.14", "unit": "kg/m^2", "unitDescription": "kilograms per square meter"}], "typeOfFlow": "Product flow", "classification": {"classHierarchy": "Kunststoffe / Dachbahnen / TPO-Dachbahnen (FPO)", "name": "OEKOBAU.DAT"}}, {"dataSetInternalID": 1, "referenceToFlowDataSet": {"shortDescription": [{"value": "Erneuerbare Primärenergie als Energieträger (PERE)", "lang": "de"}, {"value": "Renewable primary energy as energy carrier (PERE)", "lang": "en"}], "type": "flow data set", "refObjectId": "20f32be5-0398-4288-9b6d-accddd195317", "uri": "../flows/20f32be5-0398-4288-9b6d-accddd195317.xml"}, "exchange direction": "INPUT", "other": {"anies": [{"name": "referenceToUnitGroupDataSet", "value": {"shortDescription": [{"value": "MJ", "lang": "de"}], "type": "unit group data set", "refObjectId": "93a60a57-a3c8-11da-a746-0800200c9a66", "uri": "../unitgroups/93a60a57-a3c8-11da-a746-0800200c9a66.xml"}}, {"value": "11.419383367172", "module": "A1-A3"}, {"value": "0", "module": "C1"}, {"value": "0.0350665778808023", "module": "C2", "scenario": "S1"}, {"value": "0.00584442964680038", "module": "C2", "scenario": "S2"}, {"value": "1.05992947707427", "module": "C3", "scenario": "S1"}, {"value": "0.184184139464465", "module": "C3", "scenario": "S2"}, {"value": "0", "module": "C4"}, {"value": "-3.36508607370193", "module": "D", "scenario": "S1"}, {"value": "-14.8494562775088", "module": "D", "scenario": "S2"}]}, "resolvedFlowVersion": "38.00.000", "flowProperties": [], "typeOfFlow": "Other flow", "classification": {"classHierarchy": "Quantities", "name": "GaBiCategories"}}, {"dataSetInternalID": 2, "referenceToFlowDataSet": {"shortDescription": [{"value": "Erneuerbare Primärenergie zur stofflichen Nutzung (PERM)", "lang": "de"}, {"value": "Renewable primary energy resources as material utilization (PERM)", "lang": "en"}], "type": "flow data set", "refObjectId": "fb3ec0de-548d-4508-aea5-00b73bf6f702", "uri": "../flows/fb3ec0de-548d-4508-aea5-00b73bf6f702.xml"}, "exchange direction": "INPUT", "other": {"anies": [{"name": "referenceToUnitGroupDataSet", "value": {"shortDescription": [{"value": "MJ", "lang": "de"}], "type": "unit group data set", "refObjectId": "93a60a57-a3c8-11da-a746-0800200c9a66", "uri": "../unitgroups/93a60a57-a3c8-11da-a746-0800200c9a66.xml"}}, {"value": "0.74347836", "module": "A1-A3"}, {"value": "0", "module": "C1"}, {"value": "0", "module": "C2", "scenario": "S1"}, {"value": "0", "module": "C2", "scenario": "S2"}, {"value": "0", "module": "C3", "scenario": "S1"}, {"value": "0", "module": "C3", "scenario": "S2"}, {"value": "0", "module": "C4"}, {"value": "0", "module": "D", "scenario": "S1"}, {"value": "0", "module": "D", "scenario": "S2"}]}, "resolvedFlowVersion": "38.00.000", "flowProperties": [], "typeOfFlow": "Other flow", "classification": {"classHierarchy": "Quantities", "name": "GaBiCategories"}}, {"dataSetInternalID": 3, "referenceToFlowDataSet": {"shortDescription": [{"value": "Total erneuerbare Primärenergie (PERT)", "lang": "de"}, {"value": "Total use of renewable primary energy resources (PERT)", "lang": "en"}], "type": "flow data set", "refObjectId": "53f97275-fa8a-4cdd-9024-65936002acd0", "uri": "../flows/53f97275-fa8a-4cdd-9024-65936002acd0.xml"}, "exchange direction": "INPUT", "other": {"anies": [{"name": "referenceToUnitGroupDataSet", "value": {"shortDescription": [{"value": "MJ", "lang": "de"}], "type": "unit group data set", "refObjectId": "93a60a57-a3c8-11da-a746-0800200c9a66", "uri": "../unitgroups/93a60a57-a3c8-11da-a746-0800200c9a66.xml"}}, {"value": "12.162861727172", "module": "A1-A3"}, {"value": "0", "module": "C1"}, {"value": "0.0350665778808023", "module": "C2", "scenario": "S1"}, {"value": "0.00584442964680038", "module": "C2", "scenario": "S2"}, {"value": "1.05992947707427", "module": "C3", "scenario": "S1"}, {"value": "0.184184139464465", "module": "C3", "scenario": "S2"}, {"value": "0", "module": "C4"}, {"value": "-3.36508607370193", "module": "D", "scenario": "S1"}, {"value": "-14.8494562775088", "module": "D", "scenario": "S2"}]}, "resolvedFlowVersion": "38.00.000", "flowProperties": [], "typeOfFlow": "Other flow", "classification": {"classHierarchy": "Quantities / Environmental quantities / EPD EN 15804 / LCI indicators", "name": "GaBiCategories"}}, {"dataSetInternalID": 4, "referenceToFlowDataSet": {"shortDescription": [{"value": "Nicht-erneuerbare Primärenergie als Energieträger (PENRE)", "lang": "de"}, {"value": "Non renewable primary energy as energy carrier (PENRE)", "lang": "en"}], "type": "flow data set", "refObjectId": "ac857178-2b45-46ec-892a-a9a4332f0372", "uri": "../flows/ac857178-2b45-46ec-892a-a9a4332f0372.xml"}, "exchange direction": "INPUT", "other": {"anies": [{"name": "referenceToUnitGroupDataSet", "value": {"shortDescription": [{"value": "MJ", "lang": "de"}], "type": "unit group data set", "refObjectId": "93a60a57-a3c8-11da-a746-0800200c9a66", "uri": "../unitgroups/93a60a57-a3c8-11da-a746-0800200c9a66.xml"}}, {"value": "64.1611311369112", "module": "A1-A3"}, {"value": "0", "module": "C1"}, {"value": "0.507945947849469", "module": "C2", "scenario": "S1"}, {"value": "0.0846576579749115", "module": "C2", "scenario": "S2"}, {"value": "1.33164758675268", "module": "C3", "scenario": "S1"}, {"value": "67.7059217175434", "module": "C3", "scenario": "S2"}, {"value": "0", "module": "C4"}, {"value": "-149.797007768759", "module": "D", "scenario": "S1"}, {"value": "-53.7781117320027", "module": "D", "scenario": "S2"}]}, "resolvedFlowVersion": "38.00.000", "flowProperties": [], "typeOfFlow": "Other flow", "classification": {"classHierarchy": "Quantities", "name": "GaBiCategories"}}, {"dataSetInternalID": 5, "referenceToFlowDataSet": {"shortDescription": [{"value": "Nicht-erneuerbare Primärenergie zur stofflichen Nutzung (PENRM)", "lang": "de"}, {"value": "Non renewable primary energy as material utilization (PENRM)", "lang": "en"}], "type": "flow data set", "refObjectId": "1421caa0-679d-4bf4-b282-0eb850ccae27", "uri": "../flows/1421caa0-679d-4bf4-b282-0eb850ccae27.xml"}, "exchange direction": "INPUT", "other": {"anies": [{"name": "referenceToUnitGroupDataSet", "value": {"shortDescription": [{"value": "MJ", "lang": "de"}], "type": "unit group data set", "refObjectId": "93a60a57-a3c8-11da-a746-0800200c9a66", "uri": "../unitgroups/93a60a57-a3c8-11da-a746-0800200c9a66.xml"}}, {"value": "67.3099428642368", "module": "A1-A3"}, {"value": "0", "module": "C1"}, {"value": "0", "module": "C2", "scenario": "S1"}, {"value": "0", "module": "C2", "scenario": "S2"}, {"value": "0", "module": "C3", "scenario": "S1"}, {"value": "-66.9245728642369", "module": "C3", "scenario": "S2"}, {"value": "0", "module": "C4"}, {"value": "0", "module": "D", "scenario": "S1"}, {"value": "0", "module": "D", "scenario": "S2"}]}, "resolvedFlowVersion": "38.00.000", "flowProperties": [], "typeOfFlow": "Other flow", "classification": {"classHierarchy": "Quantities", "name": "GaBiCategories"}}, {"dataSetInternalID": 6, "referenceToFlowDataSet": {"shortDescription": [{"value": "Total nicht erneuerbare Primärenergie (PENRT)", "lang": "de"}, {"value": "Total use of non renewable primary energy resources (PENRT)", "lang": "en"}], "type": "flow data set", "refObjectId": "06159210-646b-4c8d-8583-da9b3b95a6c1", "uri": "../flows/06159210-646b-4c8d-8583-da9b3b95a6c1.xml"}, "exchange direction": "INPUT", "other": {"anies": [{"name": "referenceToUnitGroupDataSet", "value": {"shortDescription": [{"value": "MJ", "lang": "de"}], "type": "unit group data set", "refObjectId": "93a60a57-a3c8-11da-a746-0800200c9a66", "uri": "../unitgroups/93a60a57-a3c8-11da-a746-0800200c9a66.xml"}}, {"value": "131.471074001148", "module": "A1-A3"}, {"value": "0", "module": "C1"}, {"value": "0.507945947849469", "module": "C2", "scenario": "S1"}, {"value": "0.0846576579749115", "module": "C2", "scenario": "S2"}, {"value": "1.33164758675268", "module": "C3", "scenario": "S1"}, {"value": "0.781348853306587", "module": "C3", "scenario": "S2"}, {"value": "0", "module": "C4"}, {"value": "-149.797007768759", "module": "D", "scenario": "S1"}, {"value": "-53.7781117320027", "module": "D", "scenario": "S2"}]}, "resolvedFlowVersion": "38.00.000", "flowProperties": [], "typeOfFlow": "Other flow", "classification": {"classHierarchy": "Quantities / Environmental quantities / EPD EN 15804 / LCI indicators", "name": "GaBiCategories"}}, {"dataSetInternalID": 7, "referenceToFlowDataSet": {"shortDescription": [{"value": "Einsatz von Sekundärstoffen (SM)", "lang": "de"}, {"value": "Use of secondary material (SM)", "lang": "en"}], "type": "flow data set", "refObjectId": "c6a1f35f-2d09-4f54-8dfb-97e502e1ce92", "uri": "../flows/c6a1f35f-2d09-4f54-8dfb-97e502e1ce92.xml"}, "exchange direction": "INPUT", "other": {"anies": [{"name": "referenceToUnitGroupDataSet", "value": {"shortDescription": [{"value": "kg", "lang": "de"}], "type": "unit group data set", "refObjectId": "ad38d542-3fe9-439d-9b95-2f5f7752acaf", "uri": "../unitgroups/ad38d542-3fe9-439d-9b95-2f5f7752acaf.xml"}}, {"value": "0.039590358969151", "module": "A1-A3"}, {"value": "0", "module": "C1"}, {"value": "0", "module": "C2", "scenario": "S1"}, {"value": "0", "module": "C2", "scenario": "S2"}, {"value": "0", "module": "C3", "scenario": "S1"}, {"value": "0", "module": "C3", "scenario": "S2"}, {"value": "0", "module": "C4"}, {"value": "2.14", "module": "D", "scenario": "S1"}, {"value": "0", "module": "D", "scenario": "S2"}]}, "resolvedFlowVersion": "38.00.000", "flowProperties": [], "typeOfFlow": "Other flow", "classification": {"classHierarchy": "Quantities / Environmental quantities / EPD EN 15804 / LCI indicators", "name": "GaBiCategories"}}, {"dataSetInternalID": 8, "referenceToFlowDataSet": {"shortDescription": [{"value": "Erneuerbare Sekundärbrennstoffe (RSF)", "lang": "de"}, {"value": "Use of renewable secondary fuels (RSF)", "lang": "en"}], "type": "flow data set", "refObjectId": "64333088-a55f-4aa2-9a31-c10b07816787", "uri": "../flows/64333088-a55f-4aa2-9a31-c10b07816787.xml"}, "exchange direction": "INPUT", "other": {"anies": [{"name": "referenceToUnitGroupDataSet", "value": {"shortDescription": [{"value": "MJ", "lang": "de"}], "type": "unit group data set", "refObjectId": "93a60a57-a3c8-11da-a746-0800200c9a66", "uri": "../unitgroups/93a60a57-a3c8-11da-a746-0800200c9a66.xml"}}, {"value": "0", "module": "A1-A3"}, {"value": "0", "module": "C1"}, {"value": "0", "module": "C2", "scenario": "S1"}, {"value": "0", "module": "C2", "scenario": "S2"}, {"value": "0", "module": "C3", "scenario": "S1"}, {"value": "0", "module": "C3", "scenario": "S2"}, {"value": "0", "module": "C4"}, {"value": "0", "module": "D", "scenario": "S1"}, {"value": "0", "module": "D", "scenario": "S2"}]}, "resolvedFlowVersion": "38.00.000", "flowProperties": [], "typeOfFlow": "Other flow", "classification": {"classHierarchy": "Quantities / Environmental quantities / EPD EN 15804 / LCI indicators", "name": "GaBiCategories"}}, {"dataSetInternalID": 9, "referenceToFlowDataSet": {"shortDescription": [{"value": "Nicht erneuerbare Sekundärbrennstoffe (NRSF)", "lang": "de"}, {"value": "Use of non renewable secondary fuels (NRSF)", "lang": "en"}], "type": "flow data set", "refObjectId": "89def144-d39a-4287-b86f-efde453ddcb2", "uri": "../flows/89def144-d39a-4287-b86f-efde453ddcb2.xml"}, "exchange direction": "INPUT", "other": {"anies": [{"name": "referenceToUnitGroupDataSet", "value": {"shortDescription": [{"value": "MJ", "lang": "de"}], "type": "unit group data set", "refObjectId": "93a60a57-a3c8-11da-a746-0800200c9a66", "uri": "../unitgroups/93a60a57-a3c8-11da-a746-0800200c9a66.xml"}}, {"value": "0", "module": "A1-A3"}, {"value": "0", "module": "C1"}, {"value": "0", "module": "C2", "scenario": "S1"}, {"value": "0", "module": "C2", "scenario": "S2"}, {"value": "0", "module": "C3", "scenario": "S1"}, {"value": "0", "module": "C3", "scenario": "S2"}, {"value": "0", "module": "C4"}, {"value": "0", "module": "D", "scenario": "S1"}, {"value": "0", "module": "D", "scenario": "S2"}]}, "resolvedFlowVersion": "38.00.000", "flowProperties": [], "typeOfFlow": "Other flow", "classification": {"classHierarchy": "Quantities / Environmental quantities / EPD EN 15804 / LCI indicators", "name": "GaBiCategories"}}, {"dataSetInternalID": 10, "referenceToFlowDataSet": {"shortDescription": [{"value": "Einsatz von Süßwasserressourcen (FW)", "lang": "de"}, {"value": "Use of net fresh water (FW)", "lang": "en"}], "type": "flow data set", "refObjectId": "3cf952c8-f3a4-461d-8c96-96456ca62246", "uri": "../flows/3cf952c8-f3a4-461d-8c96-96456ca62246.xml"}, "exchange direction": "INPUT", "other": {"anies": [{"name": "referenceToUnitGroupDataSet", "value": {"shortDescription": [{"value": "m^3", "lang": "de"}], "type": "unit group data set", "refObjectId": "cd950537-0a98-4044-9ba7-9f9a68d0a504", "uri": "../unitgroups/cd950537-0a98-4044-9ba7-9f9a68d0a504.xml"}}, {"value": "0.0169015213462025", "module": "A1-A3"}, {"value": "0", "module": "C1"}, {"value": "4.05081672346713E-05", "module": "C2", "scenario": "S1"}, {"value": "6.75136120577866E-06", "module": "C2", "scenario": "S2"}, {"value": "0.000426236149161485", "module": "C3", "scenario": "S1"}, {"value": "0.0144823112179046", "module": "C3", "scenario": "S2"}, {"value": "0", "module": "C4"}, {"value": "-0.0186969624917026", "module": "D", "scenario": "S1"}, {"value": "-0.0142738738446813", "module": "D", "scenario": "S2"}]}, "resolvedFlowVersion": "38.00.000", "flowProperties": [], "typeOfFlow": "Other flow", "classification": {"classHierarchy": "Quantities / Environmental quantities / EPD EN 15804 / LCI indicators", "name": "GaBiCategories"}}, {"dataSetInternalID": 11, "referenceToFlowDataSet": {"shortDescription": [{"value": "Gefährlicher Abfall zur Deponie (HWD)", "lang": "de"}, {"value": "Hazardous waste disposed (HWD)", "lang": "en"}], "type": "flow data set", "refObjectId": "430f9e0f-59b2-46a0-8e0d-55e0e84948fc", "uri": "../flows/430f9e0f-59b2-46a0-8e0d-55e0e84948fc.xml"}, "exchange direction": "OUTPUT", "other": {"anies": [{"name": "referenceToUnitGroupDataSet", "value": {"shortDescription": [{"value": "kg", "lang": "de"}], "type": "unit group data set", "refObjectId": "ad38d542-3fe9-439d-9b95-2f5f7752acaf", "uri": "../unitgroups/ad38d542-3fe9-439d-9b95-2f5f7752acaf.xml"}}, {"value": "9.10060129417871E-06", "module": "A1-A3"}, {"value": "0", "module": "C1"}, {"value": "2.68764458002902E-12", "module": "C2", "scenario": "S1"}, {"value": "4.47940763338171E-13", "module": "C2", "scenario": "S2"}, {"value": "1.38670890492978E-10", "module": "C3", "scenario": "S1"}, {"value": "7.35132984155524E-11", "module": "C3", "scenario": "S2"}, {"value": "0", "module": "C4"}, {"value": "-7.46064375899709E-09", "module": "D", "scenario": "S1"}, {"value": "-7.26657522763226E-09", "module": "D", "scenario": "S2"}]}, "resolvedFlowVersion": "38.00.000", "flowProperties": [], "typeOfFlow": "Other flow", "classification": {"classHierarchy": "Quantities / Environmental quantities / EPD EN 15804 / LCI indicators", "name": "GaBiCategories"}}, {"dataSetInternalID": 12, "referenceToFlowDataSet": {"shortDescription": [{"value": "Entsorgter nicht gefährlicher Abfall (NHWD)", "lang": "de"}, {"value": "Non hazardous waste disposed (NHWD)", "lang": "en"}], "type": "flow data set", "refObjectId": "b29ef66b-e286-4afa-949f-62f1a7b4d7fa", "uri": "../flows/b29ef66b-e286-4afa-949f-62f1a7b4d7fa.xml"}, "exchange direction": "OUTPUT", "other": {"anies": [{"name": "referenceToUnitGroupDataSet", "value": {"shortDescription": [{"value": "kg", "lang": "de"}], "type": "unit group data set", "refObjectId": "ad38d542-3fe9-439d-9b95-2f5f7752acaf", "uri": "../unitgroups/ad38d542-3fe9-439d-9b95-2f5f7752acaf.xml"}}, {"value": "1.04289056207365", "module": "A1-A3"}, {"value": "0", "module": "C1"}, {"value": "8.27570351122103E-05", "module": "C2", "scenario": "S1"}, {"value": "1.37928391853684E-05", "module": "C2", "scenario": "S2"}, {"value": "0.00131531460763388", "module": "C3", "scenario": "S1"}, {"value": "0.0265665308249981", "module": "C3", "scenario": "S2"}, {"value": "0", "module": "C4"}, {"value": "-0.029421295252672", "module": "D", "scenario": "S1"}, {"value": "-0.0272414859211005", "module": "D", "scenario": "S2"}]}, "resolvedFlowVersion": "38.00.000", "flowProperties": [], "typeOfFlow": "Other flow", "classification": {"classHierarchy": "Quantities / Environmental quantities / EPD EN 15804 / LCI indicators", "name": "GaBiCategories"}}, {"dataSetInternalID": 13, "referenceToFlowDataSet": {"shortDescription": [{"value": "Entsorgter radioaktiver Abfall (RWD)", "lang": "de"}, {"value": "Radioactive waste disposed (RWD)", "lang": "en"}], "type": "flow data set", "refObjectId": "3449546e-52ad-4b39-b809-9fb77cea8ff6", "uri": "../flows/3449546e-52ad-4b39-b809-9fb77cea8ff6.xml"}, "exchange direction": "OUTPUT", "other": {"anies": [{"name": "referenceToUnitGroupDataSet", "value": {"shortDescription": [{"value": "kg", "lang": "de"}], "type": "unit group data set", "refObjectId": "ad38d542-3fe9-439d-9b95-2f5f7752acaf", "uri": "../unitgroups/ad38d542-3fe9-439d-9b95-2f5f7752acaf.xml"}}, {"value": "0.00197103635351463", "module": "A1-A3"}, {"value": "0", "module": "C1"}, {"value": "9.42894082919368E-07", "module": "C2", "scenario": "S1"}, {"value": "1.57149013819895E-07", "module": "C2", "scenario": "S2"}, {"value": "0.000117270961695706", "module": "C3", "scenario": "S1"}, {"value": "4.72724186361646E-05", "module": "C3", "scenario": "S2"}, {"value": "0", "module": "C4"}, {"value": "-0.000933676321578183", "module": "D", "scenario": "S1"}, {"value": "-0.00425833482708084", "module": "D", "scenario": "S2"}]}, "resolvedFlowVersion": "38.00.000", "flowProperties": [], "typeOfFlow": "Other flow", "classification": {"classHierarchy": "Quantities / Environmental quantities / EPD EN 15804 / LCI indicators", "name": "GaBiCategories"}}, {"dataSetInternalID": 14, "referenceToFlowDataSet": {"shortDescription": [{"value": "Komponenten für die Wiederverwendung (CRU)", "lang": "de"}, {"value": "Components for re-use (CRU)", "lang": "en"}], "type": "flow data set", "refObjectId": "a2b32f97-3fc7-4af2-b209-525bc6426f33", "uri": "../flows/a2b32f97-3fc7-4af2-b209-525bc6426f33.xml"}, "exchange direction": "OUTPUT", "other": {"anies": [{"name": "referenceToUnitGroupDataSet", "value": {"shortDescription": [{"value": "kg", "lang": "de"}], "type": "unit group data set", "refObjectId": "ad38d542-3fe9-439d-9b95-2f5f7752acaf", "uri": "../unitgroups/ad38d542-3fe9-439d-9b95-2f5f7752acaf.xml"}}, {"value": "0", "module": "A1-A3"}, {"value": "0", "module": "C1"}, {"value": "0", "module": "C2", "scenario": "S1"}, {"value": "0", "module": "C2", "scenario": "S2"}, {"value": "0", "module": "C3", "scenario": "S1"}, {"value": "0", "module": "C3", "scenario": "S2"}, {"value": "0", "module": "C4"}, {"value": "0", "module": "D", "scenario": "S1"}, {"value": "0", "module": "D", "scenario": "S2"}]}, "resolvedFlowVersion": "38.00.000", "flowProperties": [], "typeOfFlow": "Other flow", "classification": {"classHierarchy": "Quantities / Environmental quantities / EPD EN 15804 / LCI indicators", "name": "GaBiCategories"}}, {"dataSetInternalID": 15, "referenceToFlowDataSet": {"shortDescription": [{"value": "Stoffe zum Recycling (MFR)", "lang": "de"}, {"value": "Materials for recycling (MFR)", "lang": "en"}], "type": "flow data set", "refObjectId": "d7fe48a5-4103-49c8-9aae-b0b5dfdbd6ae", "uri": "../flows/d7fe48a5-4103-49c8-9aae-b0b5dfdbd6ae.xml"}, "exchange direction": "OUTPUT", "other": {"anies": [{"name": "referenceToUnitGroupDataSet", "value": {"shortDescription": [{"value": "kg", "lang": "de"}], "type": "unit group data set", "refObjectId": "ad38d542-3fe9-439d-9b95-2f5f7752acaf", "uri": "../unitgroups/ad38d542-3fe9-439d-9b95-2f5f7752acaf.xml"}}, {"value": "0", "module": "A1-A3"}, {"value": "0", "module": "C1"}, {"value": "0", "module": "C2", "scenario": "S1"}, {"value": "0", "module": "C2", "scenario": "S2"}, {"value": "2.14", "module": "C3", "scenario": "S1"}, {"value": "0", "module": "C3", "scenario": "S2"}, {"value": "0", "module": "C4"}, {"value": "0", "module": "D", "scenario": "S1"}, {"value": "0", "module": "D", "scenario": "S2"}]}, "resolvedFlowVersion": "38.00.000", "flowProperties": [], "typeOfFlow": "Other flow", "classification": {"classHierarchy": "Quantities / Environmental quantities / EPD EN 15804 / LCI indicators", "name": "GaBiCategories"}}, {"dataSetInternalID": 16, "referenceToFlowDataSet": {"shortDescription": [{"value": "Stoffe für die Energierückgewinnung (MER)", "lang": "de"}, {"value": "Materials for energy recovery (MER)", "lang": "en"}], "type": "flow data set", "refObjectId": "59a9181c-3aaf-46ee-8b13-2b3723b6e447", "uri": "../flows/59a9181c-3aaf-46ee-8b13-2b3723b6e447.xml"}, "exchange direction": "OUTPUT", "other": {"anies": [{"name": "referenceToUnitGroupDataSet", "value": {"shortDescription": [{"value": "kg", "lang": "de"}], "type": "unit group data set", "refObjectId": "ad38d542-3fe9-439d-9b95-2f5f7752acaf", "uri": "../unitgroups/ad38d542-3fe9-439d-9b95-2f5f7752acaf.xml"}}, {"value": "0", "module": "A1-A3"}, {"value": "0", "module": "C1"}, {"value": "0", "module": "C2", "scenario": "S1"}, {"value": "0", "module": "C2", "scenario": "S2"}, {"value": "0", "module": "C3", "scenario": "S1"}, {"value": "0", "module": "C3", "scenario": "S2"}, {"value": "0", "module": "C4"}, {"value": "0", "module": "D", "scenario": "S1"}, {"value": "0", "module": "D", "scenario": "S2"}]}, "resolvedFlowVersion": "38.00.000", "flowProperties": [], "typeOfFlow": "Other flow", "classification": {"classHierarchy": "Quantities / Environmental quantities / EPD EN 15804 / LCI indicators", "name": "GaBiCategories"}}, {"dataSetInternalID": 17, "referenceToFlowDataSet": {"shortDescription": [{"value": "Exportierte elektrische Energie (EEE)", "lang": "de"}, {"value": "Exported electrical energy (EEE)", "lang": "en"}], "type": "flow data set", "refObjectId": "4da0c987-2b76-40d6-9e9e-82a017aaaf29", "uri": "../flows/4da0c987-2b76-40d6-9e9e-82a017aaaf29.xml"}, "exchange direction": "OUTPUT", "other": {"anies": [{"name": "referenceToUnitGroupDataSet", "value": {"shortDescription": [{"value": "MJ", "lang": "de"}], "type": "unit group data set", "refObjectId": "93a60a57-a3c8-11da-a746-0800200c9a66", "uri": "../unitgroups/93a60a57-a3c8-11da-a746-0800200c9a66.xml"}}, {"value": "0", "module": "A1-A3"}, {"value": "0", "module": "C1"}, {"value": "0", "module": "C2", "scenario": "S1"}, {"value": "0", "module": "C2", "scenario": "S2"}, {"value": "0", "module": "C3", "scenario": "S1"}, {"value": "14.2976395966464", "module": "C3", "scenario": "S2"}, {"value": "0", "module": "C4"}, {"value": "0", "module": "D", "scenario": "S1"}, {"value": "0", "module": "D", "scenario": "S2"}]}, "resolvedFlowVersion": "38.00.000", "flowProperties": [], "typeOfFlow": "Other flow", "classification": {"classHierarchy": "Quantities / Environmental quantities / EPD EN 15804 / LCI indicators", "name": "GaBiCategories"}}, {"dataSetInternalID": 18, "referenceToFlowDataSet": {"shortDescription": [{"value": "Exportierte thermische Energie (EET)", "lang": "de"}, {"value": "Exported thermal energy (EET)", "lang": "en"}], "type": "flow data set", "refObjectId": "98daf38a-7a79-46d3-9a37-2b7bd0955810", "uri": "../flows/98daf38a-7a79-46d3-9a37-2b7bd0955810.xml"}, "exchange direction": "OUTPUT", "other": {"anies": [{"name": "referenceToUnitGroupDataSet", "value": {"shortDescription": [{"value": "MJ", "lang": "de"}], "type": "unit group data set", "refObjectId": "93a60a57-a3c8-11da-a746-0800200c9a66", "uri": "../unitgroups/93a60a57-a3c8-11da-a746-0800200c9a66.xml"}}, {"value": "0", "module": "A1-A3"}, {"value": "0", "module": "C1"}, {"value": "0", "module": "C2", "scenario": "S1"}, {"value": "0", "module": "C2", "scenario": "S2"}, {"value": "0", "module": "C3", "scenario": "S1"}, {"value": "25.4231675202574", "module": "C3", "scenario": "S2"}, {"value": "0", "module": "C4"}, {"value": "0", "module": "D", "scenario": "S1"}, {"value": "0", "module": "D", "scenario": "S2"}]}, "resolvedFlowVersion": "38.00.000", "flowProperties": [], "typeOfFlow": "Other flow", "classification": {"classHierarchy": "Quantities / Environmental quantities / EPD EN 15804 / LCI indicators", "name": "GaBiCategories"}}]}, "LCIAResults": {"LCIAResult": [{"referenceToLCIAMethodDataSet": {"shortDescription": [{"value": "Globales Erwärmungspotenzial total (GWP-total)", "lang": "de"}, {"value": "Global Warming Potential total (GWP-total)", "lang": "en"}], "type": "LCIA method data set", "refObjectId": "6a37f984-a4b3-458a-a20a-64418c145fa2", "uri": "../lciamethods/6a37f984-a4b3-458a-a20a-64418c145fa2.xml"}, "other": {"anies": [{"name": "referenceToUnitGroupDataSet", "value": {"shortDescription": [{"value": "kg CO_(2)-Äq.", "lang": "de"}], "type": "unit group data set", "refObjectId": "1ebf3012-d0db-4de2-aefd-ef30cedb0be1", "uri": "../unitgroups/1ebf3012-d0db-4de2-aefd-ef30cedb0be1.xml"}}, {"value": "4.73830499936557", "module": "A1-A3"}, {"value": "0", "module": "C1"}, {"value": "0.0385246693578033", "module": "C2", "scenario": "S1"}, {"value": "0.00642077822630056", "module": "C2", "scenario": "S2"}, {"value": "0.106552263158241", "module": "C3", "scenario": "S1"}, {"value": "6.70209397916524", "module": "C3", "scenario": "S2"}, {"value": "0", "module": "C4"}, {"value": "-3.73693688941553", "module": "D", "scenario": "S1"}, {"value": "-3.17705731302745", "module": "D", "scenario": "S2"}]}}, {"referenceToLCIAMethodDataSet": {"shortDescription": [{"value": "Globales Erwärmungspotenzial fossil (GWP-fossil)", "lang": "de"}, {"value": "Global Warming Potential fossil fuels (GWP-fossil)", "lang": "en"}], "type": "LCIA method data set", "refObjectId": "5f635281-343e-44fb-83df-1971b155e6b6", "uri": "../lciamethods/5f635281-343e-44fb-83df-1971b155e6b6.xml"}, "other": {"anies": [{"name": "referenceToUnitGroupDataSet", "value": {"shortDescription": [{"value": "kg CO_(2)-Äq.", "lang": "de"}], "type": "unit group data set", "refObjectId": "1ebf3012-d0db-4de2-aefd-ef30cedb0be1", "uri": "../unitgroups/1ebf3012-d0db-4de2-aefd-ef30cedb0be1.xml"}}, {"value": "4.69754640425348", "module": "A1-A3"}, {"value": "0", "module": "C1"}, {"value": "0.0382649558531493", "module": "C2", "scenario": "S1"}, {"value": "0.00637749264219155", "module": "C2", "scenario": "S2"}, {"value": "0.105171820538763", "module": "C3", "scenario": "S1"}, {"value": "6.70187165059107", "module": "C3", "scenario": "S2"}, {"value": "0", "module": "C4"}, {"value": "-3.71853129557732", "module": "D", "scenario": "S1"}, {"value": "-3.16047861939355", "module": "D", "scenario": "S2"}]}}, {"referenceToLCIAMethodDataSet": {"shortDescription": [{"value": "Globales Erwärmungspotenzial biogen (GWP-biogenic)", "lang": "de"}, {"value": "Global Warming Potential biogenic (GWP-biogenic)", "lang": "en"}], "type": "LCIA method data set", "refObjectId": "2356e1ab-0185-4db5-86e5-16de51c7485c", "uri": "../lciamethods/2356e1ab-0185-4db5-86e5-16de51c7485c.xml"}, "other": {"anies": [{"name": "referenceToUnitGroupDataSet", "value": {"shortDescription": [{"value": "kg CO_(2)-Äq.", "lang": "de"}], "type": "unit group data set", "refObjectId": "1ebf3012-d0db-4de2-aefd-ef30cedb0be1", "uri": "../unitgroups/1ebf3012-d0db-4de2-aefd-ef30cedb0be1.xml"}}, {"value": "0.0396441829206661", "module": "A1-A3"}, {"value": "0", "module": "C1"}, {"value": "0", "module": "C2", "scenario": "S1"}, {"value": "0", "module": "C2", "scenario": "S2"}, {"value": "0.00134536140802327", "module": "C3", "scenario": "S1"}, {"value": "0.000215259056730268", "module": "C3", "scenario": "S2"}, {"value": "0", "module": "C4"}, {"value": "-0.0181885456254924", "module": "D", "scenario": "S1"}, {"value": "-0.0162296584335824", "module": "D", "scenario": "S2"}]}}, {"referenceToLCIAMethodDataSet": {"shortDescription": [{"value": "Globales Erwärmungspotenzial luluc (GWP-luluc)", "lang": "de"}, {"value": "Global Warming Potential luluc (GWP-luluc)", "lang": "en"}], "type": "LCIA method data set", "refObjectId": "4331bbdb-978a-490d-8707-eeb047f01a55", "uri": "../lciamethods/4331bbdb-978a-490d-8707-eeb047f01a55.xml"}, "other": {"anies": [{"name": "referenceToUnitGroupDataSet", "value": {"shortDescription": [{"value": "kg CO_(2)-Äq.", "lang": "de"}], "type": "unit group data set", "refObjectId": "1ebf3012-d0db-4de2-aefd-ef30cedb0be1", "uri": "../unitgroups/1ebf3012-d0db-4de2-aefd-ef30cedb0be1.xml"}}, {"value": "0.00111444373342733", "module": "A1-A3"}, {"value": "0", "module": "C1"}, {"value": "0.000259713504654053", "module": "C2", "scenario": "S1"}, {"value": "4.32855841090088E-05", "module": "C2", "scenario": "S2"}, {"value": "3.50812114553865E-05", "module": "C3", "scenario": "S1"}, {"value": "7.06951744641906E-06", "module": "C3", "scenario": "S2"}, {"value": "0", "module": "C4"}, {"value": "-0.000217048212712587", "module": "D", "scenario": "S1"}, {"value": "-0.000349035200315999", "module": "D", "scenario": "S2"}]}}, {"referenceToLCIAMethodDataSet": {"shortDescription": [{"value": "Abbau Potential der stratosphärischen Ozonschicht (ODP)", "lang": "de"}, {"value": "Depletion potential of the stratospheric ozone layer (ODP)", "lang": "en"}], "type": "LCIA method data set", "refObjectId": "b5c629d6-def3-11e6-bf01-fe55135034f3", "uri": "../lciamethods/b5c629d6-def3-11e6-bf01-fe55135034f3.xml"}, "other": {"anies": [{"name": "referenceToUnitGroupDataSet", "value": {"shortDescription": [{"value": "kg CFC11-Äq.", "lang": "de"}], "type": "unit group data set", "refObjectId": "d9e957c9-7309-4474-bf3a-7777df6c4e5b", "uri": "../unitgroups/d9e957c9-7309-4474-bf3a-7777df6c4e5b.xml"}}, {"value": "2.98822544434554E-11", "module": "A1-A3"}, {"value": "0", "module": "C1"}, {"value": "3.78479828358332E-15", "module": "C2", "scenario": "S1"}, {"value": "6.30799713930553E-16", "module": "C2", "scenario": "S2"}, {"value": "2.2869063759744E-12", "module": "C3", "scenario": "S1"}, {"value": "2.8714719840366E-13", "module": "C3", "scenario": "S2"}, {"value": "0", "module": "C4"}, {"value": "-4.72719004874287E-12", "module": "D", "scenario": "S1"}, {"value": "-2.14959077432036E-11", "module": "D", "scenario": "S2"}]}}, {"referenceToLCIAMethodDataSet": {"shortDescription": [{"value": "Versauerungspotenzial von Boden und Wasser (AP)", "lang": "de"}, {"value": "Acidification potential of land and water (AP)", "lang": "en"}], "type": "LCIA method data set", "refObjectId": "b5c611c6-def3-11e6-bf01-fe55135034f3", "uri": "../lciamethods/b5c611c6-def3-11e6-bf01-fe55135034f3.xml"}, "other": {"anies": [{"name": "referenceToUnitGroupDataSet", "value": {"shortDescription": [{"value": "mol H^(+)-Äq.", "lang": "de"}], "type": "unit group data set", "refObjectId": "42e089ac-92bf-4bf2-8ca1-5fc40d18f2ed", "uri": "../unitgroups/42e089ac-92bf-4bf2-8ca1-5fc40d18f2ed.xml"}}, {"value": "0.0115505560201185", "module": "A1-A3"}, {"value": "0", "module": "C1"}, {"value": "0.000128800325668536", "module": "C2", "scenario": "S1"}, {"value": "2.14667209447561E-05", "module": "C2", "scenario": "S2"}, {"value": "0.000149065043446392", "module": "C3", "scenario": "S1"}, {"value": "0.000665409687789979", "module": "C3", "scenario": "S2"}, {"value": "0", "module": "C4"}, {"value": "-0.0072593861518961", "module": "D", "scenario": "S1"}, {"value": "-0.00417153061810069", "module": "D", "scenario": "S2"}]}}, {"referenceToLCIAMethodDataSet": {"shortDescription": [{"value": "Eutrophierungspotenzial Süßwasser (EP-freshwater)", "lang": "de"}, {"value": "Eutrophication potential aquatic freshwater (EP-freshwater)", "lang": "en"}], "type": "LCIA method data set", "refObjectId": "b53ec18f-7377-4ad3-86eb-cc3f4f276b2b", "uri": "../lciamethods/b53ec18f-7377-4ad3-86eb-cc3f4f276b2b.xml"}, "other": {"anies": [{"name": "referenceToUnitGroupDataSet", "value": {"shortDescription": [{"value": "kg P-Äq.", "lang": "de"}], "type": "unit group data set", "refObjectId": "0429039d-a61d-4590-ba67-aa4a20a810a1", "uri": "../unitgroups/0429039d-a61d-4590-ba67-aa4a20a810a1.xml"}}, {"value": "1.44071665056019E-05", "module": "A1-A3"}, {"value": "0", "module": "C1"}, {"value": "1.37681002301406E-07", "module": "C2", "scenario": "S1"}, {"value": "2.29468337169009E-08", "module": "C2", "scenario": "S2"}, {"value": "4.603794831591E-07", "module": "C3", "scenario": "S1"}, {"value": "6.69389781789988E-08", "module": "C3", "scenario": "S2"}, {"value": "0", "module": "C4"}, {"value": "-3.96626707869617E-06", "module": "D", "scenario": "S1"}, {"value": "-4.37288093772485E-06", "module": "D", "scenario": "S2"}]}}, {"referenceToLCIAMethodDataSet": {"shortDescription": [{"value": "Eutrophierungspotenzial Salzwasser (EP-marine)", "lang": "de"}, {"value": "Eutrophication potential aquatic marine (EP-marine)", "lang": "en"}], "type": "LCIA method data set", "refObjectId": "b5c619fa-def3-11e6-bf01-fe55135034f3", "uri": "../lciamethods/b5c619fa-def3-11e6-bf01-fe55135034f3.xml"}, "other": {"anies": [{"name": "referenceToUnitGroupDataSet", "value": {"shortDescription": [{"value": "kg N-Äq.", "lang": "de"}], "type": "unit group data set", "refObjectId": "d05bb823-ecdf-4686-8c40-bf1d9257859f", "uri": "../unitgroups/d05bb823-ecdf-4686-8c40-bf1d9257859f.xml"}}, {"value": "0.003089574114731", "module": "A1-A3"}, {"value": "0", "module": "C1"}, {"value": "5.88935659408594E-05", "module": "C2", "scenario": "S1"}, {"value": "9.81559432347656E-06", "module": "C2", "scenario": "S2"}, {"value": "4.79257554157432E-05", "module": "C3", "scenario": "S1"}, {"value": "0.000138760916714196", "module": "C3", "scenario": "S2"}, {"value": "0", "module": "C4"}, {"value": "-0.00195717690513616", "module": "D", "scenario": "S1"}, {"value": "-0.00113006832692076", "module": "D", "scenario": "S2"}]}}, {"referenceToLCIAMethodDataSet": {"shortDescription": [{"value": "Eutrophierungspotenzial Land (EP-terrestrial)", "lang": "de"}, {"value": "Eutrophication potential terrestrial (EP-terrestrial)", "lang": "en"}], "type": "LCIA method data set", "refObjectId": "b5c614d2-def3-11e6-bf01-fe55135034f3", "uri": "../lciamethods/b5c614d2-def3-11e6-bf01-fe55135034f3.xml"}, "other": {"anies": [{"name": "referenceToUnitGroupDataSet", "value": {"shortDescription": [{"value": "mol N-Äq.", "lang": "de"}], "type": "unit group data set", "refObjectId": "71b4d617-0ec9-4d3f-b65e-e438940c2401", "uri": "../unitgroups/71b4d617-0ec9-4d3f-b65e-e438940c2401.xml"}}, {"value": "0.0328821753087556", "module": "A1-A3"}, {"value": "0", "module": "C1"}, {"value": "0.000659600829320349", "module": "C2", "scenario": "S1"}, {"value": "0.000109933471553391", "module": "C2", "scenario": "S2"}, {"value": "0.000498817530851442", "module": "C3", "scenario": "S1"}, {"value": "0.00311721414420881", "module": "C3", "scenario": "S2"}, {"value": "0", "module": "C4"}, {"value": "-0.020928470636461", "module": "D", "scenario": "S1"}, {"value": "-0.012101307157905", "module": "D", "scenario": "S2"}]}}, {"referenceToLCIAMethodDataSet": {"shortDescription": [{"value": "Bildungspotential für troposphärisches Ozon (POCP)", "lang": "de"}, {"value": "Formation potential of tropospheric ozone photochemical oxidants (POCP)", "lang": "en"}], "type": "LCIA method data set", "refObjectId": "b5c610fe-def3-11e6-bf01-fe55135034f3", "uri": "../lciamethods/b5c610fe-def3-11e6-bf01-fe55135034f3.xml"}, "other": {"anies": [{"name": "referenceToUnitGroupDataSet", "value": {"shortDescription": [{"value": "kg NMVOC-Äq.", "lang": "de"}], "type": "unit group data set", "refObjectId": "d27c25f8-fbc1-44c6-b47b-4adbae4199c6", "uri": "../unitgroups/d27c25f8-fbc1-44c6-b47b-4adbae4199c6.xml"}}, {"value": "0.00934760924823845", "module": "A1-A3"}, {"value": "0", "module": "C1"}, {"value": "0.000115613644107643", "module": "C2", "scenario": "S1"}, {"value": "1.92689406846072E-05", "module": "C2", "scenario": "S2"}, {"value": "0.000117405126447314", "module": "C3", "scenario": "S1"}, {"value": "0.000413164679249833", "module": "C3", "scenario": "S2"}, {"value": "0", "module": "C4"}, {"value": "-0.00957051194755625", "module": "D", "scenario": "S1"}, {"value": "-0.00316197829144225", "module": "D", "scenario": "S2"}]}}, {"referenceToLCIAMethodDataSet": {"shortDescription": [{"value": "Potenzial für den abiotischen Abbau nicht fossiler Ressourcen (ADPE)", "lang": "de"}, {"value": "Abiotic depletion potential for non fossil resources (ADPE)", "lang": "en"}], "type": "LCIA method data set", "refObjectId": "b2ad6494-c78d-11e6-9d9d-cec0c932ce01", "uri": "../lciamethods/b2ad6494-c78d-11e6-9d9d-cec0c932ce01.xml"}, "other": {"anies": [{"name": "referenceToUnitGroupDataSet", "value": {"shortDescription": [{"value": "kg Sb-Äq.", "lang": "de"}], "type": "unit group data set", "refObjectId": "54ccd2d9-a32a-4fc2-923d-f2c8c93e89d4", "uri": "../unitgroups/54ccd2d9-a32a-4fc2-923d-f2c8c93e89d4.xml"}}, {"value": "1.17441875211808E-05", "module": "A1-A3"}, {"value": "0", "module": "C1"}, {"value": "3.88461330929717E-09", "module": "C2", "scenario": "S1"}, {"value": "6.47435551549528E-10", "module": "C2", "scenario": "S2"}, {"value": "4.79922023402317E-08", "module": "C3", "scenario": "S1"}, {"value": "6.95204340590011E-09", "module": "C3", "scenario": "S2"}, {"value": "0", "module": "C4"}, {"value": "-5.1159530401839E-07", "module": "D", "scenario": "S1"}, {"value": "-4.78842468117268E-07", "module": "D", "scenario": "S2"}]}}, {"referenceToLCIAMethodDataSet": {"shortDescription": [{"value": "Potenzial für den abiotischen Abbau fossiler Brennstoffe (ADPF)", "lang": "de"}, {"value": "Abiotic depletion potential for fossil resources (ADPF)", "lang": "en"}], "type": "LCIA method data set", "refObjectId": "b2ad6110-c78d-11e6-9d9d-cec0c932ce01", "uri": "../lciamethods/b2ad6110-c78d-11e6-9d9d-cec0c932ce01.xml"}, "other": {"anies": [{"name": "referenceToUnitGroupDataSet", "value": {"shortDescription": [{"value": "MJ", "lang": "de"}], "type": "unit group data set", "refObjectId": "93a60a57-a3c8-11da-a746-0800200c9a66", "uri": "../unitgroups/93a60a57-a3c8-11da-a746-0800200c9a66.xml"}}, {"value": "131.362404240881", "module": "A1-A3"}, {"value": "0", "module": "C1"}, {"value": "0.505942533524927", "module": "C2", "scenario": "S1"}, {"value": "0.0843237555874879", "module": "C2", "scenario": "S2"}, {"value": "1.33120525741571", "module": "C3", "scenario": "S1"}, {"value": "0.780719734705071", "module": "C3", "scenario": "S2"}, {"value": "0", "module": "C4"}, {"value": "-149.538381514658", "module": "D", "scenario": "S1"}, {"value": "-53.7708396325882", "module": "D", "scenario": "S2"}]}}, {"referenceToLCIAMethodDataSet": {"shortDescription": [{"value": "Wassernutzung (WDP)", "lang": "de"}, {"value": "Water use (WDP)", "lang": "en"}], "type": "LCIA method data set", "refObjectId": "b2ad66ce-c78d-11e6-9d9d-cec0c932ce01", "uri": "../lciamethods/b2ad66ce-c78d-11e6-9d9d-cec0c932ce01.xml"}, "other": {"anies": [{"name": "referenceToUnitGroupDataSet", "value": {"shortDescription": [{"value": "m^(3) Welt-Äq. entzogen", "lang": "de"}], "type": "unit group data set", "refObjectId": "6ae2df01-888e-46c8-b17d-49fa3869b476", "uri": "../unitgroups/6ae2df01-888e-46c8-b17d-49fa3869b476.xml"}}, {"value": "0.158393818744235", "module": "A1-A3"}, {"value": "0", "module": "C1"}, {"value": "0.000431214343399034", "module": "C2", "scenario": "S1"}, {"value": "7.186905723317E-05", "module": "C2", "scenario": "S2"}, {"value": "0.00242826374280775", "module": "C3", "scenario": "S1"}, {"value": "0.61830316871131", "module": "C3", "scenario": "S2"}, {"value": "0", "module": "C4"}, {"value": "-0.734057442691206", "module": "D", "scenario": "S1"}, {"value": "-0.338608804318341", "module": "D", "scenario": "S2"}]}}, {"referenceToLCIAMethodDataSet": {"shortDescription": [{"value": "Auftreten von Krankheiten aufgrund von Feinstaubemissionen (PM)", "lang": "de"}, {"value": "Incidence of disease due to PM emissions (PM)", "lang": "en"}], "type": "LCIA method data set", "refObjectId": "b5c602c6-def3-11e6-bf01-fe55135034f3", "uri": "../lciamethods/b5c602c6-def3-11e6-bf01-fe55135034f3.xml"}, "other": {"anies": [{"name": "referenceToUnitGroupDataSet", "value": {"shortDescription": [{"value": "Krankheitsfälle", "lang": "de"}], "type": "unit group data set", "refObjectId": "3883559b-648f-4afc-8ba2-0bd24f3affa3", "uri": "../unitgroups/3883559b-648f-4afc-8ba2-0bd24f3affa3.xml"}}, {"module": "A1-A3"}, {"module": "C1"}, {"module": "C2", "scenario": "S1"}, {"module": "C2", "scenario": "S2"}, {"module": "C3", "scenario": "S1"}, {"module": "C3", "scenario": "S2"}, {"module": "C4"}, {"module": "D", "scenario": "S1"}, {"module": "D", "scenario": "S2"}]}}, {"referenceToLCIAMethodDataSet": {"shortDescription": [{"value": "Wirkung durch Exposition des Menschen mit U235 (IR)", "lang": "de"}, {"value": "Human exposure efficiency relative to U235 (IR)", "lang": "en"}], "type": "LCIA method data set", "refObjectId": "b5c632be-def3-11e6-bf01-fe55135034f3", "uri": "../lciamethods/b5c632be-def3-11e6-bf01-fe55135034f3.xml"}, "other": {"anies": [{"name": "referenceToUnitGroupDataSet", "value": {"shortDescription": [{"value": "kBq U235-Äq.", "lang": "de"}], "type": "unit group data set", "refObjectId": "456b05bf-1415-44a9-9993-02452f554c09", "uri": "../unitgroups/456b05bf-1415-44a9-9993-02452f554c09.xml"}}, {"module": "A1-A3"}, {"module": "C1"}, {"module": "C2", "scenario": "S1"}, {"module": "C2", "scenario": "S2"}, {"module": "C3", "scenario": "S1"}, {"module": "C3", "scenario": "S2"}, {"module": "C4"}, {"module": "D", "scenario": "S1"}, {"module": "D", "scenario": "S2"}]}}, {"referenceToLCIAMethodDataSet": {"shortDescription": [{"value": "Toxizitätsvergleichseinheit für Ökosysteme (ETP-fw)", "lang": "de"}, {"value": "Comparative toxic unit for ecosystems (ETP-fw)", "lang": "en"}], "type": "LCIA method data set", "refObjectId": "ee1082d1-b0f7-43ca-a1f0-21e2a4a74511", "uri": "../lciamethods/ee1082d1-b0f7-43ca-a1f0-21e2a4a74511.xml"}, "other": {"anies": [{"name": "referenceToUnitGroupDataSet", "value": {"shortDescription": [{"value": "CTUe", "lang": "de"}], "type": "unit group data set", "refObjectId": "aa959ded-f1eb-4efb-9c5c-2d60be36b3e6", "uri": "../unitgroups/aa959ded-f1eb-4efb-9c5c-2d60be36b3e6.xml"}}, {"module": "A1-A3"}, {"module": "C1"}, {"module": "C2", "scenario": "S1"}, {"module": "C2", "scenario": "S2"}, {"module": "C3", "scenario": "S1"}, {"module": "C3", "scenario": "S2"}, {"module": "C4"}, {"module": "D", "scenario": "S1"}, {"module": "D", "scenario": "S2"}]}}, {"referenceToLCIAMethodDataSet": {"shortDescription": [{"value": "Toxizitätsvergleichseinheit für Menschen (krebserregend) (HTP-c)", "lang": "de"}, {"value": "Comparative toxic unit for humans (carcinogenic) (HTP-c)", "lang": "en"}], "type": "LCIA method data set", "refObjectId": "2299222a-bbd8-474f-9d4f-4dd1f18aea7c", "uri": "../lciamethods/2299222a-bbd8-474f-9d4f-4dd1f18aea7c.xml"}, "other": {"anies": [{"name": "referenceToUnitGroupDataSet", "value": {"shortDescription": [{"value": "CTUh", "lang": "de"}], "type": "unit group data set", "refObjectId": "d4c9523e-2d7e-49fd-8469-998f547d3a70", "uri": "../unitgroups/d4c9523e-2d7e-49fd-8469-998f547d3a70.xml"}}, {"module": "A1-A3"}, {"module": "C1"}, {"module": "C2", "scenario": "S1"}, {"module": "C2", "scenario": "S2"}, {"module": "C3", "scenario": "S1"}, {"module": "C3", "scenario": "S2"}, {"module": "C4"}, {"module": "D", "scenario": "S1"}, {"module": "D", "scenario": "S2"}]}}, {"referenceToLCIAMethodDataSet": {"shortDescription": [{"value": "Toxizitätsvergleichseinheit für Menschen (nicht krebserregend) (HTP-nc)", "lang": "de"}, {"value": "Comparative toxic unit for humans (noncarcinogenic) (HTP-nc)", "lang": "en"}], "type": "LCIA method data set", "refObjectId": "3af763a5-b7a1-48c9-9cee-1f223481fcef", "uri": "../lciamethods/3af763a5-b7a1-48c9-9cee-1f223481fcef.xml"}, "other": {"anies": [{"name": "referenceToUnitGroupDataSet", "value": {"shortDescription": [{"value": "CTUh", "lang": "de"}], "type": "unit group data set", "refObjectId": "d4c9523e-2d7e-49fd-8469-998f547d3a70", "uri": "../unitgroups/d4c9523e-2d7e-49fd-8469-998f547d3a70.xml"}}, {"module": "A1-A3"}, {"module": "C1"}, {"module": "C2", "scenario": "S1"}, {"module": "C2", "scenario": "S2"}, {"module": "C3", "scenario": "S1"}, {"module": "C3", "scenario": "S2"}, {"module": "C4"}, {"module": "D", "scenario": "S1"}, {"module": "D", "scenario": "S2"}]}}, {"referenceToLCIAMethodDataSet": {"shortDescription": [{"value": "Bodenqualitätsindex (SQP)", "lang": "de"}, {"value": "Soil quality index (SQP)", "lang": "en"}], "type": "LCIA method data set", "refObjectId": "b2ad6890-c78d-11e6-9d9d-cec0c932ce01", "uri": "../lciamethods/b2ad6890-c78d-11e6-9d9d-cec0c932ce01.xml"}, "other": {"anies": [{"name": "referenceToUnitGroupDataSet", "value": {"shortDescription": [{"value": "SQP", "lang": "de"}], "type": "unit group data set", "refObjectId": "f130951c-e67f-4f7f-8dd4-665de3974e18", "uri": "../unitgroups/f130951c-e67f-4f7f-8dd4-665de3974e18.xml"}}, {"module": "A1-A3"}, {"module": "C1"}, {"module": "C2", "scenario": "S1"}, {"module": "C2", "scenario": "S2"}, {"module": "C3", "scenario": "S1"}, {"module": "C3", "scenario": "S2"}, {"module": "C4"}, {"module": "D", "scenario": "S1"}, {"module": "D", "scenario": "S2"}]}}]}, "otherAttributes": {"{http://www.indata.network/EPD/2019}epd-version": "1.2"}, "version": "1.1", "locations": "../ILCDLocations.xml"}