{"processInformation": {"dataSetInformation": {"UUID": "01e17654-b05b-45a1-be19-225d34874f6d", "name": {"baseName": [{"value": "RTS 85, RTS 88, BTS 84 Series door closers", "lang": "en"}, {"value": "Türschließer der Serien RTS 85, RTS 88, BTS 84", "lang": "de"}], "functionalUnitFlowProperties": [{"lang": "en"}]}, "classificationInformation": {"classification": [{"class": [{"value": "Komponenten von Fenstern und Vorhangfassaden", "level": 0, "classId": "7"}, {"value": "Beschläge", "level": 1, "classId": "7.4"}, {"value": "Befestigungen", "level": 2, "classId": "7.4.06"}], "name": "OEKOBAU.DAT"}, {"class": [{"value": "02 Building products", "level": 0}, {"value": "Doors, windows, shutters, and related products", "level": 1}, {"value": "Building Hardware products", "level": 2}], "name": "IBUCategories"}]}, "generalComment": [{"value": "dormakaba's RTS 85, RTS 88, and BTS 84 Series concealed door closers offer a solution for installations where door control must be provided without disturbing aesthetic appearance or compromising durability. They can be installed a number of different configurations, including in standard, narrow or wide door frames, as well as with left-hand or right-hand single- or double-action mounting. The closers are designed for a wide variety of doors and represent an excellent alternative to surface-mounted closers. A comprehensive selection of accessories ensures that they can be used successfully with a wide variety of door constructions and floor coverings. Product benefits include:\n\nFor the trade: Just one body for all types of fixing. Low inventory and minimal stocking requirements thanks to unit packs for closer bodies and accessories. Reliability and a dependable design provide long-lasting performance without the visual obtrusiveness of a surface-mounted closer.\nFor the installer: Easy installation allows installers to be more productive with their time, especially because the majority of the preparation can be done prior to the installation of the unit. No floor preparation is necessary in the case of frame-mounted closers. Additionally, the \"zero\" position for double action doors is easy to adjust and closers are available with a comprehensive range of accessories.\nFor the architect: Provides an aesthetically pleasing solution, especially for toughened glass doors, and is ideal for shop fitting applications.\nFor the user: Avoids cluttering of door appearance, and backcheck prevents door contact with the frame. The closing mechanism allows for smooth performance with adjustable speed and is adjustable to accommodate traffic and weather changes.", "lang": "en"}, {"value": "Die verdeckten Türschließer der Serien RTS 85, RTS 88 und BTS 84 von dormakaba bieten eine Lösung für Installationen, bei denen die Türkontrolle ohne Beeinträchtigung des ästhetischen Erscheinungsbildes oder Kompromisse bei der Haltbarkeit gewährleistet werden muss. Sie können in verschiedenen Konfigurationen eingebaut werden, z.B. in Standard-, schmale oder breite Türrahmen, sowie mit linker oder rechter Montage mit einfacher oder doppelter Betätigung. Die Schließer sind für eine Vielzahl von Türen geeignet und stellen eine hervorragende Alternative zu aufliegenden Schließern dar. Eine umfangreiche Auswahl an Zubehör sorgt dafür, dass sie mit einer Vielzahl von Türkonstruktionen und Bodenbelägen erfolgreich eingesetzt werden können. Die Produktvorteile umfassen: Für den Handel: Ein einziger Körper für alle Arten von Befestigungen. Geringer Lagerbestand und minimale Anforderungen an die Bevorratung dank der Einheitspakete für Schließerkörper und Zubehör. Zuverlässigkeit und ein verlässliches Design sorgen für dauerhafte Leistung ohne die optische Aufdringlichkeit eines aufgesetzten Schließers. Für den Installateur: Dank der einfachen Installation können Installateure ihre Zeit produktiver nutzen, insbesondere weil der Großteil der Vorbereitungen vor der Installation des Geräts erfolgen kann. Bei rahmenmontierten Schließern ist keine Bodenvorbereitung erforderlich. Darüber hinaus lässt sich die Nullstellung bei zweiflügeligen Türen leicht einstellen und die Schließer sind mit einem umfangreichen Zubehörprogramm erhältlich. Für den Architekten: Bietet eine ästhetisch ansprechende Lösung, insbesondere für Türen aus gehärtetem Glas, und ist ideal für den Ladenbau geeignet. Für den Benutzer: Die Rücklaufsperre verhindert, dass die Tür mit dem Rahmen in Berührung kommt, und sorgt so für eine saubere Optik. Der Schließmechanismus ermöglicht einen reibungslosen Ablauf mit einstellbarer Geschwindigkeit und ist anpassbar an Verkehrs- und Wetteränderungen.", "lang": "de"}]}, "quantitativeReference": {"referenceToReferenceFlow": [0]}, "time": {"referenceYear": 2020, "dataSetValidUntil": 2025, "other": {"anies": [{"name": "publicationDateOfEPD", "value": 1598227200000}]}}, "geography": {"locationOfOperationSupplyOrProduction": {"location": "CN"}}, "technology": {"technologyDescriptionAndIncludedProcesses": [{"value": "The concealed door closers of the RTS 85, RTS 88 and BTS 84 series from dormakaba offer a solution for installations where door control must be possible without compromising on aesthetic appearance or durability. They can be installed in various configurations, e.g. in standard, narrow or wide door frames, as well as with left or right-hand mounting with single or double actuation. The closers are suitable for a wide range of doors and are an excellent alternative to surface-mounted closers. An extensive range of accessories ensures that they can be used successfully with a wide variety of door constructions and floor coverings. \nTechnical data: \nThe concealed door closers employ a cam and roller mechanism, and are capable of controlling interior and exterior doors. They are non-handed, with a single closer for both single and double-acting doors. Users can adjust closing speed and optionally take advantage of mechanical hold-open points. The plant in Suzhou is certified to the quality management system ISO 9001, which ensures consistent quality of dormakaba's products. The Environmental Management System in the Suzhou production is certified to ISO 14001. \nDeclared unit: \nThe declared unit of this analysis is one concealed door closer.", "lang": "en"}, {"value": "Die verdeckten Türschließer der Serien RTS 85, RTS 88 und BTS 84 von dormakaba bieten eine Lösung für Installationen, bei denen die Türsteuerung ohne Beeinträchtigung des ästhetischen Erscheinungsbildes oder Kompromisse bei der Haltbarkeit möglich sein muss. Sie können in verschiedenen Konfigurationen eingebaut werden, z. B. in Standard-, schmale oder breite Türrahmen, sowie mit linker oder rechter Montage mit einfacher oder doppelter Betätigung. Die Schließer sind für eine Vielzahl von Türen geeignet und stellen eine hervorragende Alternative zu aufliegenden Schließern dar. Eine umfangreiche Auswahl an Zubehör sorgt dafür, dass sie mit den unterschiedlichsten Türkonstruktionen und Bodenbelägen erfolgreich eingesetzt werden können. \nTechnische Daten: \nDie verdeckten Türschließer arbeiten mit einem Nocken- und Rollenmechanismus und können Innen- und Außentüren bedienen. Sie sind nicht bedienbar und verfügen über einen einzigen Schließer für einfach und doppelt wirkende Türen. Der Benutzer kann die Schließgeschwindigkeit einstellen und optional die Vorteile der mechanischen Feststellvorrichtung nutzen. Das Werk in Suzhou ist nach dem Qualitätsmanagementsystem ISO 9001 zertifiziert, das eine gleichbleibende Qualität der Produkte von dormakaba gewährleistet. Das Umweltmanagementsystem in der Produktion in Suzhou ist nach ISO 14001 zertifiziert. \nDeklarierte Einheit: \nDie erklärte Einheit dieser Analyse ist ein verdeckter Türschließer.", "lang": "de"}], "technologicalApplicability": [{"value": "The RTS 85, RTS 88, and BTS 84 Series offer an aesthetically pleasing solution and are well-suited for use in moveable partitions and toughened glass doors, along with aluminum, wood, and hollow metal frames. The closers can be used for retrofit applications to replace surface-mounted closers. They are not intended for use in fire or smoke doors.", "lang": "en"}, {"value": "Die Serien RTS 85, RTS 88 und BTS 84 bieten eine ästhetisch ansprechende Lösung und eignen sich gut für den Einsatz in beweglichen Trennwänden und Türen aus gehärtetem Glas sowie in Aluminium-, Holz- und Hohlmetallrahmen. Die Schließer können für Nachrüstungsanwendungen verwendet werden, um aufliegende Schließer zu ersetzen. Sie sind nicht für die Verwendung in Feuer- oder Rauchschutztüren vorgesehen.", "lang": "de"}]}}, "modellingAndValidation": {"LCIMethodAndAllocation": {"typeOfDataSet": "EPD", "referenceToLCAMethodDetails": [{"shortDescription": [{"value": "Building Hardware products.pdf", "lang": "en"}], "type": "source data set", "refObjectId": "830236f1-f03a-4ce1-91c9-601dfbb4dfa4"}], "other": {"anies": [{"name": "subType", "value": "specific dataset"}]}}, "dataSourcesTreatmentAndRepresentativeness": {"referenceToDataSource": [{"shortDescription": [{"value": "GaBi Database (all versions)", "lang": "en"}], "type": "source data set", "refObjectId": "28d74cc0-db8b-4d7e-bc44-5f6d56ce0c4a"}, {"shortDescription": [{"value": "GaBi database SP39 2019", "lang": "en"}], "type": "source data set", "refObjectId": "07d9b8a7-e0fc-408f-a95e-c90735f843ce"}], "useAdviceForDataSet": [{"value": "Scope: \nThe declaration and the background LCA represent dormakabas RTS 85, RTS 88, and BTS 84 Series Concealed Door Closers. Raw materials and components are provided by suppliers and shipped to dormakaba, where the closers are manufactured and assembled at the dormakaba facility in Suzhou, China. The RTS and BTS differ in how they are mounted to the door (floor versus frame), but are otherwise identical products. \nSystem boundary: \nType of EPD: cradle to gate - with options.\n\nThe Environmental Product Declaration refers to the production stage (A1-A3), transport from the gate to construction site (A4), the end of life stage (C3) and indicates the recycling potential which is declared in the module \"benefits and loads beyond the product system boundary\" (D).\n\nIn line with the PCR, A5 is declared to ensure the export of biogenic CO2 from renewable packaging materials.\n\nModules A1 to A3 include the provision and processing of raw materials as well as the processing of input materials, the transport to manufacturer and production site. Module C3 includes the incineration of plastics for energy recovery. Module D comprises the recycling of metals and gives\nthe recycling potentials as well as potential benefits from energy substitution.\n\nA5 is declared to ensure the export of biogenic CO2 that is incorporated in the used packaging materials (paper). Potential benefits from the incineration of packaging materials are also declared in module D. The incineration processes in the End-of-Life are based on European datasets. The recycling processes in the End-of-Life are based on European and Global datasets.", "lang": "en"}, {"value": "Gültigkeitsbereich: \nDie Deklaration und der Hintergrund der Ökobilanz beziehen sich auf die verdeckten Türschließer der Serien RTS 85, RTS 88 und BTS 84 von dormakaba. Die Rohstoffe und Komponenten werden von Lieferanten geliefert und an dormakaba verschickt, wo die Schließer im dormakaba Werk in Suzhou, China, hergestellt und montiert werden. Der RTS und der BTS unterscheiden sich in der Art und Weise, wie sie an der Tür montiert werden (Boden oder Rahmen), sind aber ansonsten identische Produkte. \nSystemgrenze: \nArt der EPD: cradle to gate - mit Optionen. Die Umweltproduktdeklaration bezieht sich auf die Produktionsstufe (A1-A3), den Transport vom Werkstor bis zur Baustelle (A4), die End-of-Life-Stufe (C3) und gibt das Recyclingpotenzial an, das im Modul \"Nutzen und Lasten über die Produktsystemgrenze hinaus\" (D) deklariert wird. In Übereinstimmung mit der PCR wird A5 deklariert, um den Export von biogenem CO2 aus erneuerbaren Verpackungsmaterialien zu gewährleisten. Die Module A1 bis A3 umfassen die Bereitstellung und Verarbeitung von Rohstoffen sowie die Verarbeitung von Vormaterialien, den Transport zum Hersteller und zur Produktionsstätte. Modul C3 umfasst die Verbrennung von Kunststoffen zur Energierückgewinnung. Modul D umfasst das Recycling von Metallen und gibt die Recyclingpotenziale sowie den potenziellen Nutzen aus der Energiesubstitution an. A5 wird angegeben, um den Export von biogenem CO2 sicherzustellen, das in den verwendeten Verpackungsmaterialien (Papier) enthalten ist. Potenzielle Vorteile aus der Verbrennung von Verpackungsmaterialien werden auch in Modul D angegeben. Die Verbrennungsprozesse im End-of-Life-Bereich basieren auf europäischen Datensätzen. Die Recyclingprozesse am Ende des Lebenszyklus basieren auf europäischen und globalen Daten.", "lang": "de"}], "other": {"anies": [{"name": "referenceToOriginalEPD", "value": {"shortDescription": {"value": "RTS 85, RTS 88, BTS 84 Series door closers.pdf", "defaultValue": "RTS 85, RTS 88, BTS 84 Series door closers.pdf", "lstrings": [{"lang": "en", "value": "RTS 85, RTS 88, BTS 84 Series door closers.pdf"}]}, "type": "source data set", "uuid": {"uuid": "c4468207-5a3c-4793-ba78-52313d70c8b2"}, "refObjectId": "c4468207-5a3c-4793-ba78-52313d70c8b2", "resourceURLs": ["https://oekobaudat.de/OEKOBAU.DAT/resource/sources/c4468207-5a3c-4793-ba78-52313d70c8b2/RTS_85_RTS_88_BTS_84_Series_door_closers_19765.pdf?version=00.01.000"]}}]}}, "validation": {"review": [{"referenceToNameOfReviewerAndInstitution": [{"shortDescription": [{"value": "Institut Bauen und Umwelt e. V.", "lang": "en"}], "type": "contact data set", "refObjectId": "d111dbec-b024-4be5-86c5-752d6eb2cf95", "uri": "../contacts/d111dbec-b024-4be5-86c5-752d6eb2cf95.xml"}], "type": "Accredited third party review"}]}, "complianceDeclarations": {"compliance": [{"referenceToComplianceSystem": {"shortDescription": [{"value": "DIN EN 15804", "lang": "en"}], "type": "source data set", "refObjectId": "b00f9ec0-7874-11e3-981f-0800200c9a66", "uri": "../sources/b00f9ec0-7874-11e3-981f-0800200c9a66.xml"}}, {"referenceToComplianceSystem": {"shortDescription": [{"value": "ISO 14025", "lang": "en"}], "type": "source data set", "refObjectId": "4f2eb655-6e44-4874-a95a-e28f5442cd4d", "uri": "../sources/4f2eb655-6e44-4874-a95a-e28f5442cd4d.xml"}}]}}, "administrativeInformation": {"commissionerAndGoal": {"referenceToCommissioner": [{"shortDescription": [{"value": "dormakaba International Holding GmbH", "lang": "en"}], "type": "contact data set", "refObjectId": "6ccc4314-c859-450c-9d21-f6ab7f69cee1", "uri": "../contacts/6ccc4314-c859-450c-9d21-f6ab7f69cee1.xml"}]}, "dataGenerator": {"referenceToPersonOrEntityGeneratingTheDataSet": [{"shortDescription": [{"value": "Sphera Solutions GmbH", "lang": "en"}], "type": "contact data set", "refObjectId": "623edf96-39d1-4e6f-9892-674c7228546b", "uri": "../contacts/623edf96-39d1-4e6f-9892-674c7228546b.xml"}]}, "dataEntryBy": {"timeStamp": 1598274624684, "referenceToDataSetFormat": [{"shortDescription": [{"value": "ILCD Format", "lang": "en"}], "type": "source data set", "refObjectId": "a97a0155-0234-4b87-b4ce-a45da52f2a40", "uri": "../sources/a97a0155-0234-4b87-b4ce-a45da52f2a40.xml"}, {"shortDescription": [{"value": "EPD-Datenformaterweiterungen v1.2", "lang": "de"}, {"value": "EPD Data Format Extensions v1.2", "lang": "en"}], "type": "source data set", "refObjectId": "a29449fd-aa2f-4de8-b5d7-4b06b43c6fde", "uri": "../sources/a29449fd-aa2f-4de8-b5d7-4b06b43c6fde.xml"}]}, "publicationAndOwnership": {"dataSetVersion": "00.01.000", "referenceToRegistrationAuthority": {"shortDescription": [{"value": "Institut Bauen und Umwelt e. V.", "lang": "en"}], "type": "contact data set", "refObjectId": "d111dbec-b024-4be5-86c5-752d6eb2cf95", "uri": "../contacts/d111dbec-b024-4be5-86c5-752d6eb2cf95.xml"}, "registrationNumber": "EPD-DOR-20200117-CBAD9-EN", "referenceToOwnershipOfDataSet": {"shortDescription": [{"value": "dormakaba International Holding GmbH", "lang": "en"}], "type": "contact data set", "refObjectId": "6ccc4314-c859-450c-9d21-f6ab7f69cee1", "uri": "../contacts/6ccc4314-c859-450c-9d21-f6ab7f69cee1.xml"}, "copyright": true, "licenseType": "Free of charge for all users and uses", "accessRestrictions": [{"value": "None", "lang": "en"}], "other": {"anies": [{"name": "referenceToPublisher", "value": {"shortDescription": [{"value": "Institut Bauen und Umwelt e. V.", "lang": "en"}], "type": "contact data set", "refObjectId": "d111dbec-b024-4be5-86c5-752d6eb2cf95", "uri": "../contacts/d111dbec-b024-4be5-86c5-752d6eb2cf95.xml"}}]}}}, "exchanges": {"exchange": [{"dataSetInternalID": 0, "referenceToFlowDataSet": {"shortDescription": [{"value": "1 closer (4.41kg) ()", "lang": "en"}], "type": "flow data set", "refObjectId": "b7777901-c193-2167-a462-72a1d6d4f5af", "uri": "../flows/b7777901-c193-2167-a462-72a1d6d4f5af.xml"}, "meanAmount": 1.0, "referencesToDataSource": {}, "referenceFlow": true, "resolvedFlowVersion": "00.01.000", "resultingflowAmount": 1.0, "flowProperties": [{"name": [{"lang": "en", "value": "Weight"}], "uuid": "93a60a56-a3c8-11da-a746-0800200b9a66", "meanValue": 4.41}, {"name": [{"lang": "de", "value": "Anzahl"}, {"lang": "en", "value": "Number of pieces"}], "uuid": "01846770-4cfe-4a25-8ad9-919d8d378345", "referenceFlowProperty": true, "meanValue": 1.0, "referenceUnit": "pcs.", "unitGroupUUID": "934110e3-baf4-49e9-992c-3d8109a6aafb"}], "materialProperties": [{"name": "weight per piece", "value": "4.41", "unit": "kg"}], "typeOfFlow": "Product flow", "classification": {"classHierarchy": "Komponenten von Fenstern und Vorhangfassaden / Beschläge / Befestigungen", "name": "OEKOBAU.DAT"}}, {"dataSetInternalID": 1, "referenceToFlowDataSet": {"shortDescription": [{"value": "Renewable primary energy as energy carrier (PERE)", "lang": "en"}, {"value": "Erneuerbare Primärenergie als Energieträger (PERE)", "lang": "de"}], "type": "flow data set", "refObjectId": "20f32be5-0398-4288-9b6d-accddd195317", "uri": "../flows/20f32be5-0398-4288-9b6d-accddd195317.xml"}, "exchange direction": "INPUT", "other": {"anies": [{"name": "referenceToUnitGroupDataSet", "value": {"shortDescription": [{"value": "MJ", "lang": "en"}], "type": "unit group data set", "refObjectId": "93a60a57-a3c8-11da-a746-0800200c9a66", "uri": "../unitgroups/93a60a57-a3c8-11da-a746-0800200c9a66.xml"}}, {"value": "29.035", "module": "A1-A3"}, {"value": "0.0658", "module": "A4"}, {"value": "3.805", "module": "A5"}, {"value": "0.0409", "module": "C3"}, {"value": "1.03", "module": "D"}]}, "resolvedFlowVersion": "38.00.000", "flowProperties": [], "typeOfFlow": "Other flow", "classification": {"classHierarchy": "Quantities", "name": "GaBiCategories"}}, {"dataSetInternalID": 2, "referenceToFlowDataSet": {"shortDescription": [{"value": "Renewable primary energy resources as material utilization (PERM)", "lang": "en"}, {"value": "Erneuerbare Primärenergie zur stofflichen Nutzung (PERM)", "lang": "de"}], "type": "flow data set", "refObjectId": "fb3ec0de-548d-4508-aea5-00b73bf6f702", "uri": "../flows/fb3ec0de-548d-4508-aea5-00b73bf6f702.xml"}, "exchange direction": "INPUT", "other": {"anies": [{"name": "referenceToUnitGroupDataSet", "value": {"shortDescription": [{"value": "MJ", "lang": "en"}], "type": "unit group data set", "refObjectId": "93a60a57-a3c8-11da-a746-0800200c9a66", "uri": "../unitgroups/93a60a57-a3c8-11da-a746-0800200c9a66.xml"}}, {"value": "3.765", "module": "A1-A3"}, {"value": "0", "module": "A4"}, {"value": "-3.765", "module": "A5"}, {"value": "0", "module": "C3"}, {"value": "0", "module": "D"}]}, "resolvedFlowVersion": "38.00.000", "flowProperties": [], "typeOfFlow": "Other flow", "classification": {"classHierarchy": "Quantities", "name": "GaBiCategories"}}, {"dataSetInternalID": 3, "referenceToFlowDataSet": {"shortDescription": [{"value": "Total use of renewable primary energy resources (PERT)", "lang": "en"}, {"value": "Total erneuerbare Primärenergie (PERT)", "lang": "de"}], "type": "flow data set", "refObjectId": "53f97275-fa8a-4cdd-9024-65936002acd0", "uri": "../flows/53f97275-fa8a-4cdd-9024-65936002acd0.xml"}, "exchange direction": "INPUT", "other": {"anies": [{"name": "referenceToUnitGroupDataSet", "value": {"shortDescription": [{"value": "MJ", "lang": "en"}], "type": "unit group data set", "refObjectId": "93a60a57-a3c8-11da-a746-0800200c9a66", "uri": "../unitgroups/93a60a57-a3c8-11da-a746-0800200c9a66.xml"}}, {"value": "32.8", "module": "A1-A3"}, {"value": "0.0658", "module": "A4"}, {"value": "0.0404", "module": "A5"}, {"value": "0.0409", "module": "C3"}, {"value": "1.03", "module": "D"}]}, "resolvedFlowVersion": "38.00.000", "flowProperties": [], "typeOfFlow": "Other flow", "classification": {"classHierarchy": "Quantities / Environmental quantities / EPD EN 15804 / LCI indicators", "name": "GaBiCategories"}}, {"dataSetInternalID": 4, "referenceToFlowDataSet": {"shortDescription": [{"value": "Non renewable primary energy as energy carrier (PENRE)", "lang": "en"}, {"value": "Nicht-erneuerbare Primärenergie als Energieträger (PENRE)", "lang": "de"}], "type": "flow data set", "refObjectId": "ac857178-2b45-46ec-892a-a9a4332f0372", "uri": "../flows/ac857178-2b45-46ec-892a-a9a4332f0372.xml"}, "exchange direction": "INPUT", "other": {"anies": [{"name": "referenceToUnitGroupDataSet", "value": {"shortDescription": [{"value": "MJ", "lang": "en"}], "type": "unit group data set", "refObjectId": "93a60a57-a3c8-11da-a746-0800200c9a66", "uri": "../unitgroups/93a60a57-a3c8-11da-a746-0800200c9a66.xml"}}, {"value": "131.17", "module": "A1-A3"}, {"value": "19.1", "module": "A4"}, {"value": "0.236", "module": "A5"}, {"value": "7.001", "module": "C3"}, {"value": "-22.7", "module": "D"}]}, "resolvedFlowVersion": "38.00.000", "flowProperties": [], "typeOfFlow": "Other flow", "classification": {"classHierarchy": "Quantities", "name": "GaBiCategories"}}, {"dataSetInternalID": 5, "referenceToFlowDataSet": {"shortDescription": [{"value": "Non renewable primary energy as material utilization (PENRM)", "lang": "en"}, {"value": "Nicht-erneuerbare Primärenergie zur stofflichen Nutzung (PENRM)", "lang": "de"}], "type": "flow data set", "refObjectId": "1421caa0-679d-4bf4-b282-0eb850ccae27", "uri": "../flows/1421caa0-679d-4bf4-b282-0eb850ccae27.xml"}, "exchange direction": "INPUT", "other": {"anies": [{"name": "referenceToUnitGroupDataSet", "value": {"shortDescription": [{"value": "MJ", "lang": "en"}], "type": "unit group data set", "refObjectId": "93a60a57-a3c8-11da-a746-0800200c9a66", "uri": "../unitgroups/93a60a57-a3c8-11da-a746-0800200c9a66.xml"}}, {"value": "6.832", "module": "A1-A3"}, {"value": "0", "module": "A4"}, {"value": "0", "module": "A5"}, {"value": "-6.832", "module": "C3"}, {"value": "0", "module": "D"}]}, "resolvedFlowVersion": "38.00.000", "flowProperties": [], "typeOfFlow": "Other flow", "classification": {"classHierarchy": "Quantities", "name": "GaBiCategories"}}, {"dataSetInternalID": 6, "referenceToFlowDataSet": {"shortDescription": [{"value": "Total use of non renewable primary energy resources (PENRT)", "lang": "en"}, {"value": "Total nicht erneuerbare Primärenergie (PENRT)", "lang": "de"}], "type": "flow data set", "refObjectId": "06159210-646b-4c8d-8583-da9b3b95a6c1", "uri": "../flows/06159210-646b-4c8d-8583-da9b3b95a6c1.xml"}, "exchange direction": "INPUT", "other": {"anies": [{"name": "referenceToUnitGroupDataSet", "value": {"shortDescription": [{"value": "MJ", "lang": "en"}], "type": "unit group data set", "refObjectId": "93a60a57-a3c8-11da-a746-0800200c9a66", "uri": "../unitgroups/93a60a57-a3c8-11da-a746-0800200c9a66.xml"}}, {"value": "138", "module": "A1-A3"}, {"value": "19.1", "module": "A4"}, {"value": "0.236", "module": "A5"}, {"value": "0.169", "module": "C3"}, {"value": "-22.7", "module": "D"}]}, "resolvedFlowVersion": "38.00.000", "flowProperties": [], "typeOfFlow": "Other flow", "classification": {"classHierarchy": "Quantities / Environmental quantities / EPD EN 15804 / LCI indicators", "name": "GaBiCategories"}}, {"dataSetInternalID": 7, "referenceToFlowDataSet": {"shortDescription": [{"value": "Use of secondary material (SM)", "lang": "en"}, {"value": "Einsatz von Sekundärstoffen (SM)", "lang": "de"}], "type": "flow data set", "refObjectId": "c6a1f35f-2d09-4f54-8dfb-97e502e1ce92", "uri": "../flows/c6a1f35f-2d09-4f54-8dfb-97e502e1ce92.xml"}, "exchange direction": "INPUT", "other": {"anies": [{"name": "referenceToUnitGroupDataSet", "value": {"shortDescription": [{"value": "kg", "lang": "en"}], "type": "unit group data set", "refObjectId": "ad38d542-3fe9-439d-9b95-2f5f7752acaf", "uri": "../unitgroups/ad38d542-3fe9-439d-9b95-2f5f7752acaf.xml"}}, {"value": "3.68", "module": "A1-A3"}, {"value": "0", "module": "A4"}, {"value": "0", "module": "A5"}, {"value": "0", "module": "C3"}, {"value": "0", "module": "D"}]}, "resolvedFlowVersion": "38.00.000", "flowProperties": [], "typeOfFlow": "Other flow", "classification": {"classHierarchy": "Quantities / Environmental quantities / EPD EN 15804 / LCI indicators", "name": "GaBiCategories"}}, {"dataSetInternalID": 8, "referenceToFlowDataSet": {"shortDescription": [{"value": "Use of renewable secondary fuels (RSF)", "lang": "en"}, {"value": "Erneuerbare Sekundärbrennstoffe (RSF)", "lang": "de"}], "type": "flow data set", "refObjectId": "64333088-a55f-4aa2-9a31-c10b07816787", "uri": "../flows/64333088-a55f-4aa2-9a31-c10b07816787.xml"}, "exchange direction": "INPUT", "other": {"anies": [{"name": "referenceToUnitGroupDataSet", "value": {"shortDescription": [{"value": "MJ", "lang": "en"}], "type": "unit group data set", "refObjectId": "93a60a57-a3c8-11da-a746-0800200c9a66", "uri": "../unitgroups/93a60a57-a3c8-11da-a746-0800200c9a66.xml"}}, {"value": "0", "module": "A1-A3"}, {"value": "0", "module": "A4"}, {"value": "0", "module": "A5"}, {"value": "0", "module": "C3"}, {"value": "0", "module": "D"}]}, "resolvedFlowVersion": "38.00.000", "flowProperties": [], "typeOfFlow": "Other flow", "classification": {"classHierarchy": "Quantities / Environmental quantities / EPD EN 15804 / LCI indicators", "name": "GaBiCategories"}}, {"dataSetInternalID": 9, "referenceToFlowDataSet": {"shortDescription": [{"value": "Use of non renewable secondary fuels (NRSF)", "lang": "en"}, {"value": "Nicht erneuerbare Sekundärbrennstoffe (NRSF)", "lang": "de"}], "type": "flow data set", "refObjectId": "89def144-d39a-4287-b86f-efde453ddcb2", "uri": "../flows/89def144-d39a-4287-b86f-efde453ddcb2.xml"}, "exchange direction": "INPUT", "other": {"anies": [{"name": "referenceToUnitGroupDataSet", "value": {"shortDescription": [{"value": "MJ", "lang": "en"}], "type": "unit group data set", "refObjectId": "93a60a57-a3c8-11da-a746-0800200c9a66", "uri": "../unitgroups/93a60a57-a3c8-11da-a746-0800200c9a66.xml"}}, {"value": "0", "module": "A1-A3"}, {"value": "0", "module": "A4"}, {"value": "0", "module": "A5"}, {"value": "0", "module": "C3"}, {"value": "0", "module": "D"}]}, "resolvedFlowVersion": "38.00.000", "flowProperties": [], "typeOfFlow": "Other flow", "classification": {"classHierarchy": "Quantities / Environmental quantities / EPD EN 15804 / LCI indicators", "name": "GaBiCategories"}}, {"dataSetInternalID": 10, "referenceToFlowDataSet": {"shortDescription": [{"value": "Use of net fresh water (FW)", "lang": "en"}, {"value": "Einsatz von Süßwasserressourcen (FW)", "lang": "de"}], "type": "flow data set", "refObjectId": "3cf952c8-f3a4-461d-8c96-96456ca62246", "uri": "../flows/3cf952c8-f3a4-461d-8c96-96456ca62246.xml"}, "exchange direction": "INPUT", "other": {"anies": [{"name": "referenceToUnitGroupDataSet", "value": {"shortDescription": [{"value": "m^3", "lang": "en"}], "type": "unit group data set", "refObjectId": "cd950537-0a98-4044-9ba7-9f9a68d0a504", "uri": "../unitgroups/cd950537-0a98-4044-9ba7-9f9a68d0a504.xml"}}, {"value": "0.0559", "module": "A1-A3"}, {"value": "0.000314", "module": "A4"}, {"value": "0.00213", "module": "A5"}, {"value": "0.000996", "module": "C3"}, {"value": "-0.00321", "module": "D"}]}, "resolvedFlowVersion": "38.00.000", "flowProperties": [], "typeOfFlow": "Other flow", "classification": {"classHierarchy": "Quantities / Environmental quantities / EPD EN 15804 / LCI indicators", "name": "GaBiCategories"}}, {"dataSetInternalID": 11, "referenceToFlowDataSet": {"shortDescription": [{"value": "Hazardous waste disposed (HWD)", "lang": "en"}, {"value": "Gefährlicher Abfall zur Deponie (HWD)", "lang": "de"}], "type": "flow data set", "refObjectId": "430f9e0f-59b2-46a0-8e0d-55e0e84948fc", "uri": "../flows/430f9e0f-59b2-46a0-8e0d-55e0e84948fc.xml"}, "exchange direction": "OUTPUT", "other": {"anies": [{"name": "referenceToUnitGroupDataSet", "value": {"shortDescription": [{"value": "kg", "lang": "en"}], "type": "unit group data set", "refObjectId": "ad38d542-3fe9-439d-9b95-2f5f7752acaf", "uri": "../unitgroups/ad38d542-3fe9-439d-9b95-2f5f7752acaf.xml"}}, {"value": "6.12E-06", "module": "A1-A3"}, {"value": "2.47E-09", "module": "A4"}, {"value": "4.57E-10", "module": "A5"}, {"value": "1.53E-09", "module": "C3"}, {"value": "-2.13E-08", "module": "D"}]}, "resolvedFlowVersion": "38.00.000", "flowProperties": [], "typeOfFlow": "Other flow", "classification": {"classHierarchy": "Quantities / Environmental quantities / EPD EN 15804 / LCI indicators", "name": "GaBiCategories"}}, {"dataSetInternalID": 12, "referenceToFlowDataSet": {"shortDescription": [{"value": "Non hazardous waste disposed (NHWD)", "lang": "en"}, {"value": "Entsorgter nicht gefährlicher Abfall (NHWD)", "lang": "de"}], "type": "flow data set", "refObjectId": "b29ef66b-e286-4afa-949f-62f1a7b4d7fa", "uri": "../flows/b29ef66b-e286-4afa-949f-62f1a7b4d7fa.xml"}, "exchange direction": "OUTPUT", "other": {"anies": [{"name": "referenceToUnitGroupDataSet", "value": {"shortDescription": [{"value": "kg", "lang": "en"}], "type": "unit group data set", "refObjectId": "ad38d542-3fe9-439d-9b95-2f5f7752acaf", "uri": "../unitgroups/ad38d542-3fe9-439d-9b95-2f5f7752acaf.xml"}}, {"value": "0.969", "module": "A1-A3"}, {"value": "0.000141", "module": "A4"}, {"value": "0.0229", "module": "A5"}, {"value": "0.0271", "module": "C3"}, {"value": "-0.0289", "module": "D"}]}, "resolvedFlowVersion": "38.00.000", "flowProperties": [], "typeOfFlow": "Other flow", "classification": {"classHierarchy": "Quantities / Environmental quantities / EPD EN 15804 / LCI indicators", "name": "GaBiCategories"}}, {"dataSetInternalID": 13, "referenceToFlowDataSet": {"shortDescription": [{"value": "Radioactive waste disposed (RWD)", "lang": "en"}, {"value": "Entsorgter radioaktiver Abfall (RWD)", "lang": "de"}], "type": "flow data set", "refObjectId": "3449546e-52ad-4b39-b809-9fb77cea8ff6", "uri": "../flows/3449546e-52ad-4b39-b809-9fb77cea8ff6.xml"}, "exchange direction": "OUTPUT", "other": {"anies": [{"name": "referenceToUnitGroupDataSet", "value": {"shortDescription": [{"value": "kg", "lang": "en"}], "type": "unit group data set", "refObjectId": "ad38d542-3fe9-439d-9b95-2f5f7752acaf", "uri": "../unitgroups/ad38d542-3fe9-439d-9b95-2f5f7752acaf.xml"}}, {"value": "0.0026", "module": "A1-A3"}, {"value": "6.5E-06", "module": "A4"}, {"value": "1.37E-05", "module": "A5"}, {"value": "6.95E-06", "module": "C3"}, {"value": "-7.2E-05", "module": "D"}]}, "resolvedFlowVersion": "38.00.000", "flowProperties": [], "typeOfFlow": "Other flow", "classification": {"classHierarchy": "Quantities / Environmental quantities / EPD EN 15804 / LCI indicators", "name": "GaBiCategories"}}, {"dataSetInternalID": 14, "referenceToFlowDataSet": {"shortDescription": [{"value": "Components for re-use (CRU)", "lang": "en"}, {"value": "Komponenten für die Wiederverwendung (CRU)", "lang": "de"}], "type": "flow data set", "refObjectId": "a2b32f97-3fc7-4af2-b209-525bc6426f33", "uri": "../flows/a2b32f97-3fc7-4af2-b209-525bc6426f33.xml"}, "exchange direction": "OUTPUT", "other": {"anies": [{"name": "referenceToUnitGroupDataSet", "value": {"shortDescription": [{"value": "kg", "lang": "en"}], "type": "unit group data set", "refObjectId": "ad38d542-3fe9-439d-9b95-2f5f7752acaf", "uri": "../unitgroups/ad38d542-3fe9-439d-9b95-2f5f7752acaf.xml"}}, {"value": "0", "module": "A1-A3"}, {"value": "0", "module": "A4"}, {"value": "0", "module": "A5"}, {"value": "0", "module": "C3"}, {"value": "0", "module": "D"}]}, "resolvedFlowVersion": "38.00.000", "flowProperties": [], "typeOfFlow": "Other flow", "classification": {"classHierarchy": "Quantities / Environmental quantities / EPD EN 15804 / LCI indicators", "name": "GaBiCategories"}}, {"dataSetInternalID": 15, "referenceToFlowDataSet": {"shortDescription": [{"value": "Materials for recycling (MFR)", "lang": "en"}, {"value": "Stoffe zum Recycling (MFR)", "lang": "de"}], "type": "flow data set", "refObjectId": "d7fe48a5-4103-49c8-9aae-b0b5dfdbd6ae", "uri": "../flows/d7fe48a5-4103-49c8-9aae-b0b5dfdbd6ae.xml"}, "exchange direction": "OUTPUT", "other": {"anies": [{"name": "referenceToUnitGroupDataSet", "value": {"shortDescription": [{"value": "kg", "lang": "en"}], "type": "unit group data set", "refObjectId": "ad38d542-3fe9-439d-9b95-2f5f7752acaf", "uri": "../unitgroups/ad38d542-3fe9-439d-9b95-2f5f7752acaf.xml"}}, {"value": "0", "module": "A1-A3"}, {"value": "0", "module": "A4"}, {"value": "0", "module": "A5"}, {"value": "1.22", "module": "C3"}, {"value": "0", "module": "D"}]}, "resolvedFlowVersion": "38.00.000", "flowProperties": [], "typeOfFlow": "Other flow", "classification": {"classHierarchy": "Quantities / Environmental quantities / EPD EN 15804 / LCI indicators", "name": "GaBiCategories"}}, {"dataSetInternalID": 16, "referenceToFlowDataSet": {"shortDescription": [{"value": "Materials for energy recovery (MER)", "lang": "en"}, {"value": "Stoffe für die Energierückgewinnung (MER)", "lang": "de"}], "type": "flow data set", "refObjectId": "59a9181c-3aaf-46ee-8b13-2b3723b6e447", "uri": "../flows/59a9181c-3aaf-46ee-8b13-2b3723b6e447.xml"}, "exchange direction": "OUTPUT", "other": {"anies": [{"name": "referenceToUnitGroupDataSet", "value": {"shortDescription": [{"value": "kg", "lang": "en"}], "type": "unit group data set", "refObjectId": "ad38d542-3fe9-439d-9b95-2f5f7752acaf", "uri": "../unitgroups/ad38d542-3fe9-439d-9b95-2f5f7752acaf.xml"}}, {"value": "0", "module": "A1-A3"}, {"value": "0", "module": "A4"}, {"value": "0", "module": "A5"}, {"value": "0", "module": "C3"}, {"value": "0", "module": "D"}]}, "resolvedFlowVersion": "38.00.000", "flowProperties": [], "typeOfFlow": "Other flow", "classification": {"classHierarchy": "Quantities / Environmental quantities / EPD EN 15804 / LCI indicators", "name": "GaBiCategories"}}, {"dataSetInternalID": 17, "referenceToFlowDataSet": {"shortDescription": [{"value": "Exported electrical energy (EEE)", "lang": "en"}, {"value": "Exportierte elektrische Energie (EEE)", "lang": "de"}], "type": "flow data set", "refObjectId": "4da0c987-2b76-40d6-9e9e-82a017aaaf29", "uri": "../flows/4da0c987-2b76-40d6-9e9e-82a017aaaf29.xml"}, "exchange direction": "OUTPUT", "other": {"anies": [{"name": "referenceToUnitGroupDataSet", "value": {"shortDescription": [{"value": "MJ", "lang": "en"}], "type": "unit group data set", "refObjectId": "93a60a57-a3c8-11da-a746-0800200c9a66", "uri": "../unitgroups/93a60a57-a3c8-11da-a746-0800200c9a66.xml"}}, {"value": "0", "module": "A1-A3"}, {"value": "0", "module": "A4"}, {"value": "1.1", "module": "A5"}, {"value": "0.248", "module": "C3"}, {"value": "0", "module": "D"}]}, "resolvedFlowVersion": "38.00.000", "flowProperties": [], "typeOfFlow": "Other flow", "classification": {"classHierarchy": "Quantities / Environmental quantities / EPD EN 15804 / LCI indicators", "name": "GaBiCategories"}}, {"dataSetInternalID": 18, "referenceToFlowDataSet": {"shortDescription": [{"value": "Exported thermal energy (EET)", "lang": "en"}, {"value": "Exportierte thermische Energie (EET)", "lang": "de"}], "type": "flow data set", "refObjectId": "98daf38a-7a79-46d3-9a37-2b7bd0955810", "uri": "../flows/98daf38a-7a79-46d3-9a37-2b7bd0955810.xml"}, "exchange direction": "OUTPUT", "other": {"anies": [{"name": "referenceToUnitGroupDataSet", "value": {"shortDescription": [{"value": "MJ", "lang": "en"}], "type": "unit group data set", "refObjectId": "93a60a57-a3c8-11da-a746-0800200c9a66", "uri": "../unitgroups/93a60a57-a3c8-11da-a746-0800200c9a66.xml"}}, {"value": "0", "module": "A1-A3"}, {"value": "0", "module": "A4"}, {"value": "2", "module": "A5"}, {"value": "0.633", "module": "C3"}, {"value": "0", "module": "D"}]}, "resolvedFlowVersion": "38.00.000", "flowProperties": [], "typeOfFlow": "Other flow", "classification": {"classHierarchy": "Quantities / Environmental quantities / EPD EN 15804 / LCI indicators", "name": "GaBiCategories"}}]}, "LCIAResults": {"LCIAResult": [{"referenceToLCIAMethodDataSet": {"shortDescription": [{"value": "Global warming potential (GWP)", "lang": "en"}, {"value": "Globales Erwärmungspotenzial (GWP)", "lang": "de"}], "type": "LCIA method data set", "refObjectId": "77e416eb-a363-4258-a04e-171d843a6460", "uri": "../lciamethods/77e416eb-a363-4258-a04e-171d843a6460.xml"}, "other": {"anies": [{"name": "referenceToUnitGroupDataSet", "value": {"shortDescription": [{"value": "kg CO_(2) eq", "lang": "en"}], "type": "unit group data set", "refObjectId": "1ebf3012-d0db-4de2-aefd-ef30cedb0be1", "uri": "../unitgroups/1ebf3012-d0db-4de2-aefd-ef30cedb0be1.xml"}}, {"value": "11.4", "module": "A1-A3"}, {"value": "1.47", "module": "A4"}, {"value": "0.728", "module": "A5"}, {"value": "0.223", "module": "C3"}, {"value": "-2.57", "module": "D"}]}}, {"referenceToLCIAMethodDataSet": {"shortDescription": [{"value": "Depletion potential of the stratospheric ozone layer (ODP)", "lang": "en"}, {"value": "Abbau Potential der stratosphärischen Ozonschicht (ODP)", "lang": "de"}], "type": "LCIA method data set", "refObjectId": "06dcd26f-025f-401a-a7c1-5e457eb54637", "uri": "../lciamethods/06dcd26f-025f-401a-a7c1-5e457eb54637.xml"}, "other": {"anies": [{"name": "referenceToUnitGroupDataSet", "value": {"shortDescription": [{"value": "kg CFC11 eq", "lang": "en"}], "type": "unit group data set", "refObjectId": "88054749-b0a6-47ea-a82b-dc5b29326512", "uri": "../unitgroups/88054749-b0a6-47ea-a82b-dc5b29326512.xml"}}, {"value": "8.59E-12", "module": "A1-A3"}, {"value": "1.12E-16", "module": "A4"}, {"value": "1.75E-16", "module": "A5"}, {"value": "2.38E-16", "module": "C3"}, {"value": "6.07E-15", "module": "D"}]}}, {"referenceToLCIAMethodDataSet": {"shortDescription": [{"value": "Acidification potential of land and water (AP)", "lang": "en"}, {"value": "Versauerungspotenzial von Boden und Wasser (AP)", "lang": "de"}], "type": "LCIA method data set", "refObjectId": "b4274add-93b7-4905-a5e4-2e878c4e4216", "uri": "../lciamethods/b4274add-93b7-4905-a5e4-2e878c4e4216.xml"}, "other": {"anies": [{"name": "referenceToUnitGroupDataSet", "value": {"shortDescription": [{"value": "kg SO_(2) eq", "lang": "en"}], "type": "unit group data set", "refObjectId": "bc50c624-a9bc-45b1-a9b0-e6b10d00476f", "uri": "../unitgroups/bc50c624-a9bc-45b1-a9b0-e6b10d00476f.xml"}}, {"value": "0.0326", "module": "A1-A3"}, {"value": "0.0399", "module": "A4"}, {"value": "0.000152", "module": "A5"}, {"value": "4.9E-05", "module": "C3"}, {"value": "-0.00577", "module": "D"}]}}, {"referenceToLCIAMethodDataSet": {"shortDescription": [{"value": "Eutrophication potential (EP)", "lang": "en"}, {"value": "Eutrophierungspotenzial (EP)", "lang": "de"}], "type": "LCIA method data set", "refObjectId": "f58827d0-b407-4ec6-be75-8b69efb98a0f", "uri": "../lciamethods/f58827d0-b407-4ec6-be75-8b69efb98a0f.xml"}, "other": {"anies": [{"name": "referenceToUnitGroupDataSet", "value": {"shortDescription": [{"value": "kg PO_(4)^(3) eq", "lang": "en"}], "type": "unit group data set", "refObjectId": "67b5401d-873c-485f-bcf3-6ae83b918822", "uri": "../unitgroups/67b5401d-873c-485f-bcf3-6ae83b918822.xml"}}, {"value": "0.00296", "module": "A1-A3"}, {"value": "0.00437", "module": "A4"}, {"value": "2.87E-05", "module": "A5"}, {"value": "1.06E-05", "module": "C3"}, {"value": "-0.000526", "module": "D"}]}}, {"referenceToLCIAMethodDataSet": {"shortDescription": [{"value": "Formation potential of tropospheric ozone photochemical oxidants (POCP)", "lang": "en"}, {"value": "Bildungspotential für troposphärisches Ozon (POCP)", "lang": "de"}], "type": "LCIA method data set", "refObjectId": "1e84a202-dae6-42aa-9e9d-71ea48b8be00", "uri": "../lciamethods/1e84a202-dae6-42aa-9e9d-71ea48b8be00.xml"}, "other": {"anies": [{"name": "referenceToUnitGroupDataSet", "value": {"shortDescription": [{"value": "kg Ethen eq", "lang": "en"}], "type": "unit group data set", "refObjectId": "01c26c17-9a76-406e-8295-f17b55fd909e", "uri": "../unitgroups/01c26c17-9a76-406e-8295-f17b55fd909e.xml"}}, {"value": "0.00409", "module": "A1-A3"}, {"value": "0.00174", "module": "A4"}, {"value": "1.01E-05", "module": "A5"}, {"value": "3.77E-06", "module": "C3"}, {"value": "-0.00073", "module": "D"}]}}, {"referenceToLCIAMethodDataSet": {"shortDescription": [{"value": "Abiotic depletion potential for non fossil resources (ADPE)", "lang": "en"}, {"value": "Potenzial für den abiotischen Abbau nicht fossiler Ressourcen (ADPE)", "lang": "de"}], "type": "LCIA method data set", "refObjectId": "f7c73bb9-ab1a-4249-9c6d-379a0de6f67e", "uri": "../lciamethods/f7c73bb9-ab1a-4249-9c6d-379a0de6f67e.xml"}, "other": {"anies": [{"name": "referenceToUnitGroupDataSet", "value": {"shortDescription": [{"value": "kg Sb eq", "lang": "en"}], "type": "unit group data set", "refObjectId": "54ccd2d9-a32a-4fc2-923d-f2c8c93e89d4", "uri": "../unitgroups/54ccd2d9-a32a-4fc2-923d-f2c8c93e89d4.xml"}}, {"value": "7.46E-05", "module": "A1-A3"}, {"value": "4.81E-08", "module": "A4"}, {"value": "1.43E-08", "module": "A5"}, {"value": "3.85E-08", "module": "C3"}, {"value": "-6.42E-06", "module": "D"}]}}, {"referenceToLCIAMethodDataSet": {"shortDescription": [{"value": "Abiotic depletion potential for fossil resources (ADPF)", "lang": "en"}, {"value": "Potenzial für den abiotischen Abbau fossiler Brennstoffe (ADPF)", "lang": "de"}], "type": "LCIA method data set", "refObjectId": "804ebcdf-309d-4098-8ed8-fdaf2f389981", "uri": "../lciamethods/804ebcdf-309d-4098-8ed8-fdaf2f389981.xml"}, "other": {"anies": [{"name": "referenceToUnitGroupDataSet", "value": {"shortDescription": [{"value": "MJ", "lang": "en"}], "type": "unit group data set", "refObjectId": "93a60a57-a3c8-11da-a746-0800200c9a66", "uri": "../unitgroups/93a60a57-a3c8-11da-a746-0800200c9a66.xml"}}, {"value": "131", "module": "A1-A3"}, {"value": "19", "module": "A4"}, {"value": "0.202", "module": "A5"}, {"value": "0.151", "module": "C3"}, {"value": "-22.5", "module": "D"}]}}]}, "otherAttributes": {"{http://www.indata.network/EPD/2019}epd-version": "1.2"}, "version": "1.1", "locations": "../ILCDLocations.xml"}