{"processInformation": {"dataSetInformation": {"UUID": "0f651489-6c74-42af-b30f-ea03249b1e5b", "name": {"baseName": [{"value": "Kvadrat Acoustics Track", "lang": "en"}, {"value": "Kvadrat Acoustics Track", "lang": "de"}], "functionalUnitFlowProperties": [{"lang": "en"}]}, "classificationInformation": {"classification": [{"class": [{"value": "Komposite", "level": 0, "classId": "10"}, {"value": "Systembauteile", "level": 1, "classId": "10.1"}, {"value": "Innenwände", "level": 2, "classId": "10.1.04"}], "name": "OEKOBAU.DAT"}, {"class": [{"value": "02 Building products", "level": 0}, {"value": "Interior facilitys", "level": 1}, {"value": "Textile covered acoustic frame systems", "level": 2}], "name": "IBUCategories"}]}, "generalComment": [{"value": "Kvadrat Acoustics Track with ABS profile and Trevira CS CASA textile is a site-fabricated acoustical wall system, which stretches textile over semi-rigid acoustic padding to control sound and add to the aesthetic design of interior spaces. The product is available in customized sizes and different textile options under the trade name Kvadrat Acoustics Track. This EPD includes only the Kvadrat Acoustics Track with ABS frame and Trevira CS textile CASA. The product is declared as a construction product 'kit', since it consists of multiple separate components and is placed on the market by a single manufacturer. The system consists of a single-sided layer of tensioned textile, attached to an ABS frame profile, over a mineral-based acoustic core.", "lang": "en"}, {"value": "Kvadrat Acoustics Track ist ein vor ort gefertigtes akustikwandsystem, das textil über eine halbstarre akustikpolsterung spannt, um den schall zu kontrollieren und zur ästhetischen gestaltung von innenräumen beizutragen. Das produkt wird als bauprodukt „bausatz“ deklariert, da es aus mehreren separaten komponenten besteht und von einem einzigen hersteller in verkehr gebracht wird.", "lang": "de"}]}, "quantitativeReference": {"referenceToReferenceFlow": [0]}, "time": {"referenceYear": 2024, "dataSetValidUntil": 2029, "other": {"anies": [{"name": "publicationDateOfEPD", "value": 1717977600000}]}}, "geography": {"locationOfOperationSupplyOrProduction": {"location": "RER"}}, "technology": {"technologyDescriptionAndIncludedProcesses": [{"value": "The Kvadrat Acoustics Track system consists of an ABS frame, a layer of mineral glass wool absorber, Trevira CS textile CASA (polyester textile) for the panel's wear, and installation staples (galvanised steel). The ABS profilesare manufactured by a supplier in Illinois, in United States of America. The rest of components are manufactured by Kvadrat Acoustics suppliers, located in Europe. The components are delivered to Kvadrat Acoustics site in the United Kingdom, where they are stored temporarily and assembled into a kit before transported to the application site (United Kingdom). The components are not considered as a kit before they reach the warehouse exit gate. \nTechnical data: \nThe product has a sound adsorption class C according to ISO 11654 with a sound absorption coefficient of 0.6 (ISO 354). The fire performance is C-s2,d0. The dimensions of the system after its installation in the building site are:\n\nTypical size panel: 2700 mm x 1300 mm x 25 mm\nMin. size panel: 1000 mm x 1000 mm x 25 mm\nMax. size panel: 6000 mm x 3000 mm x 25 mm\n\nThe components comprising the product kit are delivered at the building site with the following dimensions. The components arrive at the building site in fixed dimensions however, the number of component pieces differs across systems with different sizes.\n\nABS frame (profiles): 2700 mm x 26 mm x 23 mm\nMineral glass wool absorber: 1200 mm x 1200 mm x 22 mm\nTrevira CS CASA textile (roll): 400 mm x 400 mm x 1500 mm \nDeclared unit: \nThe declared unit is 1 m2 configurable acoustic frame system with weight of 2.79 kg/m2. The final LCA results refer to a typical Kvadrat Acoustics Track size of 2700 mm x 1300 mm x 25 mm (L x W x H), which represents all the product sizes included in this EPD. All Kvadrat Acoustics Track sizes, included in this EPD, consist of the same type of components and no variation takes place regarding the components type. The amount of each component per declared unit differs between different product sizes. No component was included as an unweighted average. The results correspond to a typical Kvadrat Acoustics Track size of 1300 mm x 2700 mm x 25 mm (L x W x H), which represents all the product sizes included in this EPD. Finally, this EPD covers only the Trevira CS textile option CASA, which is a polyester textile.", "lang": "en"}, {"value": "Das Kvadrat Acoustics Track system besteht aus einem ABS-rahmen, einer schicht mineralwollabsorber und Trevira CS-Textil CASA (polyestertextil) für den verschleiß der Platte. Montageklammern (verzinkter stahl) sind im Kit enthalten. Das ABS-rahmenprofil wird von einem zulieferer in Illinois, Vereinigte Staaten von Amerika, hergestellt. Die restlichen komponenten werden von Kvadrat Acoustics-zulieferern in Europa hergestellt. Die Komponenten werden an den standort von Kvadrat Acoustics im vereinigten Königreich geliefert, wo sie vorübergehend gelagert und zu einem bausatz zusammengebaut werden, bevor sie zum einsatzort im vereinigten Königreich transportiert werden. Die Komponenten gelten erst dann als bausatz, wenn sie das ausgangstor des lagers erreichen. \nTechnische Daten: \nKvadrat Acoustics Track haben eine schallabsorptionsklasse C und einen schallabsorptionskoeffizienten von 0,6, basierend auf ISO 11654 bzw. ISO 354. Das brandverhalten des systems beträgt C-s2,d0 gemäß EN 13501-1. Schließlich betragen die abmessungen des systems bei Installation an einer wand 2700 mm x 1300 mm x 25 mm für ein panel in typischer größe. Für eine maximale plattengröße betragen die abmessungen 6000 mm x 3000 mm x 25 mm, während sie für eine minimale Größe 1000 mm x 1000 mm x 25 mm betragen. \nDeklarierte Einheit: \nDie deklarierte einheit ist 1 m2 konfigurierbares akustikrahmensystem. ", "lang": "de"}], "technologicalApplicability": [{"value": "Kvadrat Acoustics Track controls sound and adds to the aesthetic design of interior spaces. The system is intended for interior walls and is particularly well suited for spaces with severe to moderate need for sound absorption, large free wall surfaces, and late changes as the tracks are built on-site. It is installed directly on a wall substrate and can be applied in many different markets, architectural needs and acoustic environments.", "lang": "en"}, {"value": "Kvadrat Acoustics Track steuern den klang und tragen zur ästhetischen gestaltung von innenräumen bei. Das system ist für Innenwände vorgesehen und eignet sich besonders gut für räume mit starkem bis mittlerem bedarf an schallabsorption, großen freien wandflächen und nachträglichen anderungen, da die gleise vor ort gebaut werden.", "lang": "de"}]}}, "modellingAndValidation": {"LCIMethodAndAllocation": {"typeOfDataSet": "EPD", "referenceToLCAMethodDetails": [{"shortDescription": [{"value": "Textile covered acoustic frame systems.pdf", "lang": "en"}], "type": "source data set", "refObjectId": "b81e8e6e-e32a-4a0f-b045-c11b42c8ee0b"}], "other": {"anies": [{"name": "subType", "value": "average dataset"}]}}, "dataSourcesTreatmentAndRepresentativeness": {"referenceToDataSource": [{"shortDescription": [{"value": "GaBi Database (all versions)", "lang": "en"}], "type": "source data set", "refObjectId": "28d74cc0-db8b-4d7e-bc44-5f6d56ce0c4a"}, {"shortDescription": [{"value": "GaBi Database Edition 2022, CUP 2022.02", "lang": "en"}], "type": "source data set", "refObjectId": "94f442cb-662e-43ea-a792-4b0a35132e93"}], "useAdviceForDataSet": [{"value": "Scope: \nThe declaration covers the average product Kvadrat Acoustics Track with an ABS frame and the Trevira CS textile option CASA. The Kvadrat Acoustics Track is a configurable textile-covered acoustic frame system from the company Kvadrat Acoustics. It is available with an ABS frame in customized sizes ranging from 1000 mm x 1000 mm x 25 mm to 6000 mm x 3000 mm x 25 mm (L x W x H) and the textile option CASA under the textile series Trevira CS. The product is declared as a kit since it is available by a single manufacturer as a set of multiple separate components, which are assembled at the building site. All products included in this average EPD are produced in Kvadrat Acoustics site in United Kingdom and distributed to the market of the United Kingdom. The products' components (including the Trevira CS textile CASA) are manufactured by Kvadrat Acoustics suppliers located in United States of America (Illinois) and Europe (Germany, Czech Republic, United Kingdom). Production data were collected for the year 2022. \nSystem boundary: \nThe EPD is of the type cradle-to-gate with options, modules A4, A5, C1-C4 and D. The product stage (A1-A3) includes:\nA1 - Raw material extraction, processing, processing of secondary material input (e.g. recycling processes) and production of the components. The production of excess components to compensate for material losses during the installation phase, as well as the production of ancillary materials (installation screws), are accounted for in module A1 because the product is declared as a kit.\nA2 - Transport of components and packaging from the suppliers to Kvadrat Acoustics site.\nA3 - Assembly of components into a product kit. The production of sales packaging (plastic, core board, corrugated cardboard tubes, steel end-caps packaging for the textile and frame) is included in module A3.\n\nThe construction process stage (A4-A5) includes:\nA4 - Transport of the kit from Kvadrat Acoustics site to the building site. \nA5 - Installation of Kvadrat Acoustics Track system at the application site including in-situ processing of components (cutting the components to the correct size, installing the staples). Module A5 also includes the transport and processing of waste (material loss, packaging) generated in the application site.\n\nThe end-of-life stage includes:\nC1 - Deconstruction and dismantling of the system. The manual dismantling impact of the system is considered negligible and module C1 is reported without any impacts.\nC2 - Transport of waste from the building site to Material Recovery Facilities (MRF), as well as transport of recyclable and non-recyclable waste from MRF to recycling facilities and landfill, respectively.\nC3 - Waste processing for dismantling the system into components and sorting the components/materials to waste for material recovery and landfill.\nC4 - Disposal of non-recyclable components/materials (textile, absorber) to landfill.\nModule D includes reuse, recovery and/or recycling potentials. Benefits originating from the recycling of material loss and metal components after reaching their end-of-life stage, as well as the incineration of plastic packaging, were considered in module D", "lang": "en"}, {"value": "Gültigkeitsbereich: \nDie erklärung bezieht sich auf ein modell eines konfigurierbaren textilbespannten akustikrahmensystems von Kvadrat Acoustics. Das modell heißt Kvadrat Acoustics Track mit ABS-rahmen. Das produkt wird als bausatz deklariert, da es bei einem hersteller als set aus mehreren einzelteilen erhältlich ist, die auf der Baustelle zusammengebaut werden. Die produktionsdaten wurden für 2022 – 2023 erhoben. \nSystemgrenze: \nDie EPD ist vom typ \"cradle-to-gate\" mit optionen, module A4, A5, C1-C4 und D.", "lang": "de"}], "other": {"anies": [{"name": "referenceToOriginalEPD", "value": {"shortDescription": {"value": "Kvadrat Acoustics Track.pdf", "defaultValue": "Kvadrat Acoustics Track.pdf", "lstrings": [{"lang": "en", "value": "Kvadrat Acoustics Track.pdf"}]}, "type": "source data set", "uuid": {"uuid": "36dc3623-4c33-4e95-8640-3cbcad0f02d5"}, "refObjectId": "36dc3623-4c33-4e95-8640-3cbcad0f02d5", "resourceURLs": ["https://oekobaudat.de/OEKOBAU.DAT/resource/sources/36dc3623-4c33-4e95-8640-3cbcad0f02d5/Kvadrat_Acoustics_Track_19343.pdf?version=00.01.000"]}}]}}, "validation": {"review": [{"referenceToNameOfReviewerAndInstitution": [{"shortDescription": [{"value": "Institut Bauen und Umwelt e. V.", "lang": "en"}], "type": "contact data set", "refObjectId": "d111dbec-b024-4be5-86c5-752d6eb2cf95", "uri": "../contacts/d111dbec-b024-4be5-86c5-752d6eb2cf95.xml"}], "type": "Accredited third party review"}]}, "complianceDeclarations": {"compliance": [{"referenceToComplianceSystem": {"shortDescription": [{"value": "DIN EN 15804+A2", "lang": "en"}], "type": "source data set", "refObjectId": "c0016b33-8cf7-415c-ac6e-deba0d21440d", "uri": "../sources/c0016b33-8cf7-415c-ac6e-deba0d21440d.xml"}}, {"referenceToComplianceSystem": {"shortDescription": [{"value": "ISO 14025", "lang": "en"}], "type": "source data set", "refObjectId": "4f2eb655-6e44-4874-a95a-e28f5442cd4d", "uri": "../sources/4f2eb655-6e44-4874-a95a-e28f5442cd4d.xml"}}]}}, "administrativeInformation": {"commissionerAndGoal": {"referenceToCommissioner": [{"shortDescription": [{"value": "Kvadrat Acoustics A/S", "lang": "en"}], "type": "contact data set", "refObjectId": "81df5e64-5b70-4352-aff7-345ca5f2692c", "uri": "../contacts/81df5e64-5b70-4352-aff7-345ca5f2692c.xml"}]}, "dataGenerator": {"referenceToPersonOrEntityGeneratingTheDataSet": [{"shortDescription": [{"value": "FORCE Technology", "lang": "en"}], "type": "contact data set", "refObjectId": "827dee6d-fd7f-4856-a4e8-0b3be8abfe6c", "uri": "../contacts/827dee6d-fd7f-4856-a4e8-0b3be8abfe6c.xml"}]}, "dataEntryBy": {"timeStamp": 1717977600000, "referenceToDataSetFormat": [{"shortDescription": [{"value": "ILCD Format", "lang": "en"}], "type": "source data set", "refObjectId": "a97a0155-0234-4b87-b4ce-a45da52f2a40", "uri": "../sources/a97a0155-0234-4b87-b4ce-a45da52f2a40.xml"}, {"shortDescription": [{"value": "EPD-Datenformaterweiterungen v1.2", "lang": "de"}, {"value": "EPD Data Format Extensions v1.2", "lang": "en"}], "type": "source data set", "refObjectId": "a29449fd-aa2f-4de8-b5d7-4b06b43c6fde", "uri": "../sources/a29449fd-aa2f-4de8-b5d7-4b06b43c6fde.xml"}]}, "publicationAndOwnership": {"dataSetVersion": "00.02.000", "referenceToRegistrationAuthority": {"shortDescription": [{"value": "Institut Bauen und Umwelt e. V.", "lang": "en"}], "type": "contact data set", "refObjectId": "d111dbec-b024-4be5-86c5-752d6eb2cf95", "uri": "../contacts/d111dbec-b024-4be5-86c5-752d6eb2cf95.xml"}, "registrationNumber": "EPD-KVC-20240080-CBA1-EN", "referenceToOwnershipOfDataSet": {"shortDescription": [{"value": "Kvadrat Acoustics A/S", "lang": "en"}], "type": "contact data set", "refObjectId": "81df5e64-5b70-4352-aff7-345ca5f2692c", "uri": "../contacts/81df5e64-5b70-4352-aff7-345ca5f2692c.xml"}, "copyright": true, "licenseType": "Free of charge for all users and uses", "accessRestrictions": [{"value": "None", "lang": "en"}], "other": {"anies": [{"name": "referenceToPublisher", "value": {"shortDescription": [{"value": "Institut Bauen und Umwelt e. V.", "lang": "en"}], "type": "contact data set", "refObjectId": "d111dbec-b024-4be5-86c5-752d6eb2cf95", "uri": "../contacts/d111dbec-b024-4be5-86c5-752d6eb2cf95.xml"}}]}}}, "exchanges": {"exchange": [{"dataSetInternalID": 0, "referenceToFlowDataSet": {"shortDescription": [{"value": "Kvadrat Acoustics Track (Kvadrat Acoustics Track)", "lang": "en"}], "type": "flow data set", "refObjectId": "e1180647-8930-45ee-61fa-67996024e50b", "uri": "../flows/e1180647-8930-45ee-61fa-67996024e50b.xml"}, "meanAmount": 1.0, "referencesToDataSource": {}, "referenceFlow": true, "resolvedFlowVersion": "00.02.000", "resultingflowAmount": 1.0, "flowProperties": [{"name": [{"lang": "de", "value": "Fläche"}, {"lang": "en", "value": "Area"}], "uuid": "93a60a56-a3c8-19da-a746-0800200c9a66", "referenceFlowProperty": true, "meanValue": 1.0, "referenceUnit": "qm", "unitGroupUUID": "c20a03d7-bd90-4569-bc94-66cfd364dfc8"}], "materialProperties": [{"name": "layer thickness", "value": "0.025", "unit": "m", "unitDescription": "meters"}, {"name": "grammage", "value": "2.79", "unit": "kg/m^2", "unitDescription": "kilograms per square meter"}], "typeOfFlow": "Product flow", "classification": {"classHierarchy": "Komposite / Systembauteile / Innenwände", "name": "OEKOBAU.DAT"}}, {"dataSetInternalID": 1, "referenceToFlowDataSet": {"shortDescription": [{"value": "Renewable primary energy as energy carrier (PERE)", "lang": "en"}, {"value": "Erneuerbare Primärenergie als Energieträger (PERE)", "lang": "de"}], "type": "flow data set", "refObjectId": "20f32be5-0398-4288-9b6d-accddd195317", "uri": "../flows/20f32be5-0398-4288-9b6d-accddd195317.xml"}, "exchange direction": "INPUT", "other": {"anies": [{"name": "referenceToUnitGroupDataSet", "value": {"shortDescription": [{"value": "MJ", "lang": "en"}], "type": "unit group data set", "refObjectId": "93a60a57-a3c8-11da-a746-0800200c9a66", "uri": "../unitgroups/93a60a57-a3c8-11da-a746-0800200c9a66.xml"}}, {"value": "17.9498008046791", "module": "A1"}, {"value": "0.230581495967225", "module": "A2"}, {"value": "1.96839087409879", "module": "A3"}, {"value": "0.101758075798022", "module": "A4"}, {"value": "0.0676197260091363", "module": "A5"}, {"value": "0", "module": "C1"}, {"value": "0.107856430186926", "module": "C2"}, {"value": "0.063824344110871", "module": "C3"}, {"value": "0.0838880041679744", "module": "C4"}, {"value": "-2.77213036989796", "module": "D"}]}, "resolvedFlowVersion": "38.00.000", "flowProperties": [], "typeOfFlow": "Other flow", "classification": {"classHierarchy": "Quantities", "name": "GaBiCategories"}}, {"dataSetInternalID": 2, "referenceToFlowDataSet": {"shortDescription": [{"value": "Renewable primary energy resources as material utilization (PERM)", "lang": "en"}, {"value": "Erneuerbare Primärenergie zur stofflichen Nutzung (PERM)", "lang": "de"}], "type": "flow data set", "refObjectId": "fb3ec0de-548d-4508-aea5-00b73bf6f702", "uri": "../flows/fb3ec0de-548d-4508-aea5-00b73bf6f702.xml"}, "exchange direction": "INPUT", "other": {"anies": [{"name": "referenceToUnitGroupDataSet", "value": {"shortDescription": [{"value": "MJ", "lang": "en"}], "type": "unit group data set", "refObjectId": "93a60a57-a3c8-11da-a746-0800200c9a66", "uri": "../unitgroups/93a60a57-a3c8-11da-a746-0800200c9a66.xml"}}, {"value": "3.01107086406405", "module": "A1"}, {"value": "0", "module": "A2"}, {"value": "1.7023335", "module": "A3"}, {"value": "0", "module": "A4"}, {"value": "0", "module": "A5"}, {"value": "0", "module": "C1"}, {"value": "0", "module": "C2"}, {"value": "0", "module": "C3"}, {"value": "0", "module": "C4"}, {"value": "0", "module": "D"}]}, "resolvedFlowVersion": "38.00.000", "flowProperties": [], "typeOfFlow": "Other flow", "classification": {"classHierarchy": "Quantities", "name": "GaBiCategories"}}, {"dataSetInternalID": 3, "referenceToFlowDataSet": {"shortDescription": [{"value": "Total use of renewable primary energy resources (PERT)", "lang": "en"}, {"value": "Total erneuerbare Primärenergie (PERT)", "lang": "de"}], "type": "flow data set", "refObjectId": "53f97275-fa8a-4cdd-9024-65936002acd0", "uri": "../flows/53f97275-fa8a-4cdd-9024-65936002acd0.xml"}, "exchange direction": "INPUT", "other": {"anies": [{"name": "referenceToUnitGroupDataSet", "value": {"shortDescription": [{"value": "MJ", "lang": "en"}], "type": "unit group data set", "refObjectId": "93a60a57-a3c8-11da-a746-0800200c9a66", "uri": "../unitgroups/93a60a57-a3c8-11da-a746-0800200c9a66.xml"}}, {"value": "20.9608716687432", "module": "A1"}, {"value": "0.230581495967225", "module": "A2"}, {"value": "3.67072437409879", "module": "A3"}, {"value": "0.101758075798022", "module": "A4"}, {"value": "0.0676197260091363", "module": "A5"}, {"value": "0", "module": "C1"}, {"value": "0.107856430186926", "module": "C2"}, {"value": "0.063824344110871", "module": "C3"}, {"value": "0.0838880041679744", "module": "C4"}, {"value": "-2.77213036989796", "module": "D"}]}, "resolvedFlowVersion": "38.00.000", "flowProperties": [], "typeOfFlow": "Other flow", "classification": {"classHierarchy": "Quantities / Environmental quantities / EPD EN 15804 / LCI indicators", "name": "GaBiCategories"}}, {"dataSetInternalID": 4, "referenceToFlowDataSet": {"shortDescription": [{"value": "Non renewable primary energy as energy carrier (PENRE)", "lang": "en"}, {"value": "Nicht-erneuerbare Primärenergie als Energieträger (PENRE)", "lang": "de"}], "type": "flow data set", "refObjectId": "ac857178-2b45-46ec-892a-a9a4332f0372", "uri": "../flows/ac857178-2b45-46ec-892a-a9a4332f0372.xml"}, "exchange direction": "INPUT", "other": {"anies": [{"name": "referenceToUnitGroupDataSet", "value": {"shortDescription": [{"value": "MJ", "lang": "en"}], "type": "unit group data set", "refObjectId": "93a60a57-a3c8-11da-a746-0800200c9a66", "uri": "../unitgroups/93a60a57-a3c8-11da-a746-0800200c9a66.xml"}}, {"value": "109.860115023026", "module": "A1"}, {"value": "3.6967878934232", "module": "A2"}, {"value": "3.86640359041165", "module": "A3"}, {"value": "1.40355440447009", "module": "A4"}, {"value": "0.561634550598958", "module": "A5"}, {"value": "0", "module": "C1"}, {"value": "1.4876693220866", "module": "C2"}, {"value": "14.5688398147678", "module": "C3"}, {"value": "0.593029833952464", "module": "C4"}, {"value": "-11.532813437211", "module": "D"}]}, "resolvedFlowVersion": "38.00.000", "flowProperties": [], "typeOfFlow": "Other flow", "classification": {"classHierarchy": "Quantities", "name": "GaBiCategories"}}, {"dataSetInternalID": 5, "referenceToFlowDataSet": {"shortDescription": [{"value": "Non renewable primary energy as material utilization (PENRM)", "lang": "en"}, {"value": "Nicht-erneuerbare Primärenergie zur stofflichen Nutzung (PENRM)", "lang": "de"}], "type": "flow data set", "refObjectId": "1421caa0-679d-4bf4-b282-0eb850ccae27", "uri": "../flows/1421caa0-679d-4bf4-b282-0eb850ccae27.xml"}, "exchange direction": "INPUT", "other": {"anies": [{"name": "referenceToUnitGroupDataSet", "value": {"shortDescription": [{"value": "MJ", "lang": "en"}], "type": "unit group data set", "refObjectId": "93a60a57-a3c8-11da-a746-0800200c9a66", "uri": "../unitgroups/93a60a57-a3c8-11da-a746-0800200c9a66.xml"}}, {"value": "19.0352088073908", "module": "A1"}, {"value": "0", "module": "A2"}, {"value": "0.153555", "module": "A3"}, {"value": "0", "module": "A4"}, {"value": "0", "module": "A5"}, {"value": "0", "module": "C1"}, {"value": "0", "module": "C2"}, {"value": "-14.167764", "module": "C3"}, {"value": "0", "module": "C4"}, {"value": "0", "module": "D"}]}, "resolvedFlowVersion": "38.00.000", "flowProperties": [], "typeOfFlow": "Other flow", "classification": {"classHierarchy": "Quantities", "name": "GaBiCategories"}}, {"dataSetInternalID": 6, "referenceToFlowDataSet": {"shortDescription": [{"value": "Total use of non renewable primary energy resources (PENRT)", "lang": "en"}, {"value": "Total nicht erneuerbare Primärenergie (PENRT)", "lang": "de"}], "type": "flow data set", "refObjectId": "06159210-646b-4c8d-8583-da9b3b95a6c1", "uri": "../flows/06159210-646b-4c8d-8583-da9b3b95a6c1.xml"}, "exchange direction": "INPUT", "other": {"anies": [{"name": "referenceToUnitGroupDataSet", "value": {"shortDescription": [{"value": "MJ", "lang": "en"}], "type": "unit group data set", "refObjectId": "93a60a57-a3c8-11da-a746-0800200c9a66", "uri": "../unitgroups/93a60a57-a3c8-11da-a746-0800200c9a66.xml"}}, {"value": "128.895592855827", "module": "A1"}, {"value": "3.6967878934232", "module": "A2"}, {"value": "4.02026464481485", "module": "A3"}, {"value": "1.40355440447009", "module": "A4"}, {"value": "0.561639242996203", "module": "A5"}, {"value": "0", "module": "C1"}, {"value": "1.4876693220866", "module": "C2"}, {"value": "0.401075814767765", "module": "C3"}, {"value": "0.593029833952466", "module": "C4"}, {"value": "-11.5328134372109", "module": "D"}]}, "resolvedFlowVersion": "38.00.000", "flowProperties": [], "typeOfFlow": "Other flow", "classification": {"classHierarchy": "Quantities / Environmental quantities / EPD EN 15804 / LCI indicators", "name": "GaBiCategories"}}, {"dataSetInternalID": 7, "referenceToFlowDataSet": {"shortDescription": [{"value": "Use of secondary material (SM)", "lang": "en"}, {"value": "Einsatz von Sekundärstoffen (SM)", "lang": "de"}], "type": "flow data set", "refObjectId": "c6a1f35f-2d09-4f54-8dfb-97e502e1ce92", "uri": "../flows/c6a1f35f-2d09-4f54-8dfb-97e502e1ce92.xml"}, "exchange direction": "INPUT", "other": {"anies": [{"name": "referenceToUnitGroupDataSet", "value": {"shortDescription": [{"value": "kg", "lang": "en"}], "type": "unit group data set", "refObjectId": "ad38d542-3fe9-439d-9b95-2f5f7752acaf", "uri": "../unitgroups/ad38d542-3fe9-439d-9b95-2f5f7752acaf.xml"}}, {"value": "1.24564", "module": "A1"}, {"value": "0", "module": "A2"}, {"value": "0.0715512", "module": "A3"}, {"value": "0", "module": "A4"}, {"value": "0", "module": "A5"}, {"value": "0", "module": "C1"}, {"value": "0", "module": "C2"}, {"value": "0", "module": "C3"}, {"value": "0", "module": "C4"}, {"value": "0", "module": "D"}]}, "resolvedFlowVersion": "38.00.000", "flowProperties": [], "typeOfFlow": "Other flow", "classification": {"classHierarchy": "Quantities / Environmental quantities / EPD EN 15804 / LCI indicators", "name": "GaBiCategories"}}, {"dataSetInternalID": 8, "referenceToFlowDataSet": {"shortDescription": [{"value": "Use of renewable secondary fuels (RSF)", "lang": "en"}, {"value": "Erneuerbare Sekundärbrennstoffe (RSF)", "lang": "de"}], "type": "flow data set", "refObjectId": "64333088-a55f-4aa2-9a31-c10b07816787", "uri": "../flows/64333088-a55f-4aa2-9a31-c10b07816787.xml"}, "exchange direction": "INPUT", "other": {"anies": [{"name": "referenceToUnitGroupDataSet", "value": {"shortDescription": [{"value": "MJ", "lang": "en"}], "type": "unit group data set", "refObjectId": "93a60a57-a3c8-11da-a746-0800200c9a66", "uri": "../unitgroups/93a60a57-a3c8-11da-a746-0800200c9a66.xml"}}, {"value": "0", "module": "A1"}, {"value": "0", "module": "A2"}, {"value": "0", "module": "A3"}, {"value": "0", "module": "A4"}, {"value": "0", "module": "A5"}, {"value": "0", "module": "C1"}, {"value": "0", "module": "C2"}, {"value": "0", "module": "C3"}, {"value": "0", "module": "C4"}, {"value": "0", "module": "D"}]}, "resolvedFlowVersion": "38.00.000", "flowProperties": [], "typeOfFlow": "Other flow", "classification": {"classHierarchy": "Quantities / Environmental quantities / EPD EN 15804 / LCI indicators", "name": "GaBiCategories"}}, {"dataSetInternalID": 9, "referenceToFlowDataSet": {"shortDescription": [{"value": "Use of non renewable secondary fuels (NRSF)", "lang": "en"}, {"value": "Nicht erneuerbare Sekundärbrennstoffe (NRSF)", "lang": "de"}], "type": "flow data set", "refObjectId": "89def144-d39a-4287-b86f-efde453ddcb2", "uri": "../flows/89def144-d39a-4287-b86f-efde453ddcb2.xml"}, "exchange direction": "INPUT", "other": {"anies": [{"name": "referenceToUnitGroupDataSet", "value": {"shortDescription": [{"value": "MJ", "lang": "en"}], "type": "unit group data set", "refObjectId": "93a60a57-a3c8-11da-a746-0800200c9a66", "uri": "../unitgroups/93a60a57-a3c8-11da-a746-0800200c9a66.xml"}}, {"value": "0", "module": "A1"}, {"value": "0", "module": "A2"}, {"value": "0", "module": "A3"}, {"value": "0", "module": "A4"}, {"value": "0", "module": "A5"}, {"value": "0", "module": "C1"}, {"value": "0", "module": "C2"}, {"value": "0", "module": "C3"}, {"value": "0", "module": "C4"}, {"value": "0", "module": "D"}]}, "resolvedFlowVersion": "38.00.000", "flowProperties": [], "typeOfFlow": "Other flow", "classification": {"classHierarchy": "Quantities / Environmental quantities / EPD EN 15804 / LCI indicators", "name": "GaBiCategories"}}, {"dataSetInternalID": 10, "referenceToFlowDataSet": {"shortDescription": [{"value": "Use of net fresh water (FW)", "lang": "en"}, {"value": "Einsatz von Süßwasserressourcen (FW)", "lang": "de"}], "type": "flow data set", "refObjectId": "3cf952c8-f3a4-461d-8c96-96456ca62246", "uri": "../flows/3cf952c8-f3a4-461d-8c96-96456ca62246.xml"}, "exchange direction": "INPUT", "other": {"anies": [{"name": "referenceToUnitGroupDataSet", "value": {"shortDescription": [{"value": "m^3", "lang": "en"}], "type": "unit group data set", "refObjectId": "cd950537-0a98-4044-9ba7-9f9a68d0a504", "uri": "../unitgroups/cd950537-0a98-4044-9ba7-9f9a68d0a504.xml"}}, {"value": "0.0309200692882348", "module": "A1"}, {"value": "0.00025934587272774", "module": "A2"}, {"value": "0.00206565063212261", "module": "A3"}, {"value": "0.000111452518546645", "module": "A4"}, {"value": "9.79062698856573E-05", "module": "A5"}, {"value": "0", "module": "C1"}, {"value": "0.000118131860213666", "module": "C2"}, {"value": "0.00235489022616423", "module": "C3"}, {"value": "0.000131195594657029", "module": "C4"}, {"value": "-0.0016004750836339", "module": "D"}]}, "resolvedFlowVersion": "38.00.000", "flowProperties": [], "typeOfFlow": "Other flow", "classification": {"classHierarchy": "Quantities / Environmental quantities / EPD EN 15804 / LCI indicators", "name": "GaBiCategories"}}, {"dataSetInternalID": 11, "referenceToFlowDataSet": {"shortDescription": [{"value": "Hazardous waste disposed (HWD)", "lang": "en"}, {"value": "Gefährlicher Abfall zur Deponie (HWD)", "lang": "de"}], "type": "flow data set", "refObjectId": "430f9e0f-59b2-46a0-8e0d-55e0e84948fc", "uri": "../flows/430f9e0f-59b2-46a0-8e0d-55e0e84948fc.xml"}, "exchange direction": "OUTPUT", "other": {"anies": [{"name": "referenceToUnitGroupDataSet", "value": {"shortDescription": [{"value": "kg", "lang": "en"}], "type": "unit group data set", "refObjectId": "ad38d542-3fe9-439d-9b95-2f5f7752acaf", "uri": "../unitgroups/ad38d542-3fe9-439d-9b95-2f5f7752acaf.xml"}}, {"value": "8.30773105339237E-06", "module": "A1"}, {"value": "1.12072981488188E-11", "module": "A2"}, {"value": "1.02741057167382E-08", "module": "A3"}, {"value": "4.34584985523979E-12", "module": "A4"}, {"value": "5.88886818160673E-12", "module": "A5"}, {"value": "0", "module": "C1"}, {"value": "4.60629633411015E-12", "module": "C2"}, {"value": "2.2225261998274E-11", "module": "C3"}, {"value": "2.38079627253507E-11", "module": "C4"}, {"value": "-1.82625672253637E-07", "module": "D"}]}, "resolvedFlowVersion": "38.00.000", "flowProperties": [], "typeOfFlow": "Other flow", "classification": {"classHierarchy": "Quantities / Environmental quantities / EPD EN 15804 / LCI indicators", "name": "GaBiCategories"}}, {"dataSetInternalID": 12, "referenceToFlowDataSet": {"shortDescription": [{"value": "Non hazardous waste disposed (NHWD)", "lang": "en"}, {"value": "Entsorgter nicht gefährlicher Abfall (NHWD)", "lang": "de"}], "type": "flow data set", "refObjectId": "b29ef66b-e286-4afa-949f-62f1a7b4d7fa", "uri": "../flows/b29ef66b-e286-4afa-949f-62f1a7b4d7fa.xml"}, "exchange direction": "OUTPUT", "other": {"anies": [{"name": "referenceToUnitGroupDataSet", "value": {"shortDescription": [{"value": "kg", "lang": "en"}], "type": "unit group data set", "refObjectId": "ad38d542-3fe9-439d-9b95-2f5f7752acaf", "uri": "../unitgroups/ad38d542-3fe9-439d-9b95-2f5f7752acaf.xml"}}, {"value": "0.242885040293786", "module": "A1"}, {"value": "0.00050620862296239", "module": "A2"}, {"value": "0.0256547300331578", "module": "A3"}, {"value": "0.000213956637916296", "module": "A4"}, {"value": "0.00165710423621983", "module": "A5"}, {"value": "0", "module": "C1"}, {"value": "0.000226779044311458", "module": "C2"}, {"value": "0.0241160236882311", "module": "C3"}, {"value": "2.21530396290214", "module": "C4"}, {"value": "-0.00169036488461685", "module": "D"}]}, "resolvedFlowVersion": "38.00.000", "flowProperties": [], "typeOfFlow": "Other flow", "classification": {"classHierarchy": "Quantities / Environmental quantities / EPD EN 15804 / LCI indicators", "name": "GaBiCategories"}}, {"dataSetInternalID": 13, "referenceToFlowDataSet": {"shortDescription": [{"value": "Radioactive waste disposed (RWD)", "lang": "en"}, {"value": "Entsorgter radioaktiver Abfall (RWD)", "lang": "de"}], "type": "flow data set", "refObjectId": "3449546e-52ad-4b39-b809-9fb77cea8ff6", "uri": "../flows/3449546e-52ad-4b39-b809-9fb77cea8ff6.xml"}, "exchange direction": "OUTPUT", "other": {"anies": [{"name": "referenceToUnitGroupDataSet", "value": {"shortDescription": [{"value": "kg", "lang": "en"}], "type": "unit group data set", "refObjectId": "ad38d542-3fe9-439d-9b95-2f5f7752acaf", "uri": "../unitgroups/ad38d542-3fe9-439d-9b95-2f5f7752acaf.xml"}}, {"value": "0.00360653717654871", "module": "A1"}, {"value": "7.28452600017637E-06", "module": "A2"}, {"value": "0.000177196668556186", "module": "A3"}, {"value": "2.62666858695033E-06", "module": "A4"}, {"value": "2.29794393564564E-05", "module": "A5"}, {"value": "0", "module": "C1"}, {"value": "2.78408465225819E-06", "module": "C2"}, {"value": "1.16947206668534E-05", "module": "C3"}, {"value": "6.83768139658427E-06", "module": "C4"}, {"value": "-0.000487384438160239", "module": "D"}]}, "resolvedFlowVersion": "38.00.000", "flowProperties": [], "typeOfFlow": "Other flow", "classification": {"classHierarchy": "Quantities / Environmental quantities / EPD EN 15804 / LCI indicators", "name": "GaBiCategories"}}, {"dataSetInternalID": 14, "referenceToFlowDataSet": {"shortDescription": [{"value": "Components for re-use (CRU)", "lang": "en"}, {"value": "Komponenten für die Wiederverwendung (CRU)", "lang": "de"}], "type": "flow data set", "refObjectId": "a2b32f97-3fc7-4af2-b209-525bc6426f33", "uri": "../flows/a2b32f97-3fc7-4af2-b209-525bc6426f33.xml"}, "exchange direction": "OUTPUT", "other": {"anies": [{"name": "referenceToUnitGroupDataSet", "value": {"shortDescription": [{"value": "kg", "lang": "en"}], "type": "unit group data set", "refObjectId": "ad38d542-3fe9-439d-9b95-2f5f7752acaf", "uri": "../unitgroups/ad38d542-3fe9-439d-9b95-2f5f7752acaf.xml"}}, {"value": "0", "module": "A1"}, {"value": "0", "module": "A2"}, {"value": "0", "module": "A3"}, {"value": "0", "module": "A4"}, {"value": "0", "module": "A5"}, {"value": "0", "module": "C1"}, {"value": "0", "module": "C2"}, {"value": "0", "module": "C3"}, {"value": "0", "module": "C4"}, {"value": "0", "module": "D"}]}, "resolvedFlowVersion": "38.00.000", "flowProperties": [], "typeOfFlow": "Other flow", "classification": {"classHierarchy": "Quantities / Environmental quantities / EPD EN 15804 / LCI indicators", "name": "GaBiCategories"}}, {"dataSetInternalID": 15, "referenceToFlowDataSet": {"shortDescription": [{"value": "Materials for recycling (MFR)", "lang": "en"}, {"value": "Stoffe zum Recycling (MFR)", "lang": "de"}], "type": "flow data set", "refObjectId": "d7fe48a5-4103-49c8-9aae-b0b5dfdbd6ae", "uri": "../flows/d7fe48a5-4103-49c8-9aae-b0b5dfdbd6ae.xml"}, "exchange direction": "OUTPUT", "other": {"anies": [{"name": "referenceToUnitGroupDataSet", "value": {"shortDescription": [{"value": "kg", "lang": "en"}], "type": "unit group data set", "refObjectId": "ad38d542-3fe9-439d-9b95-2f5f7752acaf", "uri": "../unitgroups/ad38d542-3fe9-439d-9b95-2f5f7752acaf.xml"}}, {"value": "0", "module": "A1"}, {"value": "0", "module": "A2"}, {"value": "0.192997143", "module": "A3"}, {"value": "0", "module": "A4"}, {"value": "0.18162431010423", "module": "A5"}, {"value": "0", "module": "C1"}, {"value": "0", "module": "C2"}, {"value": "0.16792022792", "module": "C3"}, {"value": "0", "module": "C4"}, {"value": "0", "module": "D"}]}, "resolvedFlowVersion": "38.00.000", "flowProperties": [], "typeOfFlow": "Other flow", "classification": {"classHierarchy": "Quantities / Environmental quantities / EPD EN 15804 / LCI indicators", "name": "GaBiCategories"}}, {"dataSetInternalID": 16, "referenceToFlowDataSet": {"shortDescription": [{"value": "Materials for energy recovery (MER)", "lang": "en"}, {"value": "Stoffe für die Energierückgewinnung (MER)", "lang": "de"}], "type": "flow data set", "refObjectId": "59a9181c-3aaf-46ee-8b13-2b3723b6e447", "uri": "../flows/59a9181c-3aaf-46ee-8b13-2b3723b6e447.xml"}, "exchange direction": "OUTPUT", "other": {"anies": [{"name": "referenceToUnitGroupDataSet", "value": {"shortDescription": [{"value": "kg", "lang": "en"}], "type": "unit group data set", "refObjectId": "ad38d542-3fe9-439d-9b95-2f5f7752acaf", "uri": "../unitgroups/ad38d542-3fe9-439d-9b95-2f5f7752acaf.xml"}}, {"value": "0", "module": "A1"}, {"value": "0", "module": "A2"}, {"value": "0", "module": "A3"}, {"value": "0", "module": "A4"}, {"value": "0", "module": "A5"}, {"value": "0", "module": "C1"}, {"value": "0", "module": "C2"}, {"value": "0.363276", "module": "C3"}, {"value": "0", "module": "C4"}, {"value": "0", "module": "D"}]}, "resolvedFlowVersion": "38.00.000", "flowProperties": [], "typeOfFlow": "Other flow", "classification": {"classHierarchy": "Quantities / Environmental quantities / EPD EN 15804 / LCI indicators", "name": "GaBiCategories"}}, {"dataSetInternalID": 17, "referenceToFlowDataSet": {"shortDescription": [{"value": "Exported electrical energy (EEE)", "lang": "en"}, {"value": "Exportierte elektrische Energie (EEE)", "lang": "de"}], "type": "flow data set", "refObjectId": "4da0c987-2b76-40d6-9e9e-82a017aaaf29", "uri": "../flows/4da0c987-2b76-40d6-9e9e-82a017aaaf29.xml"}, "exchange direction": "OUTPUT", "other": {"anies": [{"name": "referenceToUnitGroupDataSet", "value": {"shortDescription": [{"value": "MJ", "lang": "en"}], "type": "unit group data set", "refObjectId": "93a60a57-a3c8-11da-a746-0800200c9a66", "uri": "../unitgroups/93a60a57-a3c8-11da-a746-0800200c9a66.xml"}}, {"value": "0", "module": "A1"}, {"value": "0", "module": "A2"}, {"value": "0", "module": "A3"}, {"value": "0", "module": "A4"}, {"value": "0", "module": "A5"}, {"value": "0", "module": "C1"}, {"value": "0", "module": "C2"}, {"value": "2.20987042764783", "module": "C3"}, {"value": "0", "module": "C4"}, {"value": "0", "module": "D"}]}, "resolvedFlowVersion": "38.00.000", "flowProperties": [], "typeOfFlow": "Other flow", "classification": {"classHierarchy": "Quantities / Environmental quantities / EPD EN 15804 / LCI indicators", "name": "GaBiCategories"}}, {"dataSetInternalID": 18, "referenceToFlowDataSet": {"shortDescription": [{"value": "Exported thermal energy (EET)", "lang": "en"}, {"value": "Exportierte thermische Energie (EET)", "lang": "de"}], "type": "flow data set", "refObjectId": "98daf38a-7a79-46d3-9a37-2b7bd0955810", "uri": "../flows/98daf38a-7a79-46d3-9a37-2b7bd0955810.xml"}, "exchange direction": "OUTPUT", "other": {"anies": [{"name": "referenceToUnitGroupDataSet", "value": {"shortDescription": [{"value": "MJ", "lang": "en"}], "type": "unit group data set", "refObjectId": "93a60a57-a3c8-11da-a746-0800200c9a66", "uri": "../unitgroups/93a60a57-a3c8-11da-a746-0800200c9a66.xml"}}, {"value": "0", "module": "A1"}, {"value": "0", "module": "A2"}, {"value": "0", "module": "A3"}, {"value": "0", "module": "A4"}, {"value": "0", "module": "A5"}, {"value": "0", "module": "C1"}, {"value": "0", "module": "C2"}, {"value": "4.02290058135506", "module": "C3"}, {"value": "0", "module": "C4"}, {"value": "0", "module": "D"}]}, "resolvedFlowVersion": "38.00.000", "flowProperties": [], "typeOfFlow": "Other flow", "classification": {"classHierarchy": "Quantities / Environmental quantities / EPD EN 15804 / LCI indicators", "name": "GaBiCategories"}}]}, "LCIAResults": {"LCIAResult": [{"referenceToLCIAMethodDataSet": {"shortDescription": [{"value": "Global Warming Potential total (GWP-total)", "lang": "en"}, {"value": "Globales Erwärmungspotenzial total (GWP-total)", "lang": "de"}], "type": "LCIA method data set", "refObjectId": "6a37f984-a4b3-458a-a20a-64418c145fa2", "uri": "../lciamethods/6a37f984-a4b3-458a-a20a-64418c145fa2.xml"}, "other": {"anies": [{"name": "referenceToUnitGroupDataSet", "value": {"shortDescription": [{"value": "kg CO_(2) eq", "lang": "en"}], "type": "unit group data set", "refObjectId": "1ebf3012-d0db-4de2-aefd-ef30cedb0be1", "uri": "../unitgroups/1ebf3012-d0db-4de2-aefd-ef30cedb0be1.xml"}}, {"value": "6.32294420330716", "module": "A1"}, {"value": "0.272813874828559", "module": "A2"}, {"value": "0.00946861252855745", "module": "A3"}, {"value": "0.10214499247276", "module": "A4"}, {"value": "0.250246070056453", "module": "A5"}, {"value": "0", "module": "C1"}, {"value": "0.108595774620686", "module": "C2"}, {"value": "0.774659669566184", "module": "C3"}, {"value": "0.251428663624759", "module": "C4"}, {"value": "-0.778771441135984", "module": "D"}]}}, {"referenceToLCIAMethodDataSet": {"shortDescription": [{"value": "Global Warming Potential fossil fuels (GWP-fossil)", "lang": "en"}, {"value": "Globales Erwärmungspotenzial fossil (GWP-fossil)", "lang": "de"}], "type": "LCIA method data set", "refObjectId": "5f635281-343e-44fb-83df-1971b155e6b6", "uri": "../lciamethods/5f635281-343e-44fb-83df-1971b155e6b6.xml"}, "other": {"anies": [{"name": "referenceToUnitGroupDataSet", "value": {"shortDescription": [{"value": "kg CO_(2) eq", "lang": "en"}], "type": "unit group data set", "refObjectId": "1ebf3012-d0db-4de2-aefd-ef30cedb0be1", "uri": "../unitgroups/1ebf3012-d0db-4de2-aefd-ef30cedb0be1.xml"}}, {"value": "6.56650289607628", "module": "A1"}, {"value": "0.271261005676656", "module": "A2"}, {"value": "0.25978215032228", "module": "A3"}, {"value": "0.101473898546913", "module": "A4"}, {"value": "0.0385522459466037", "module": "A5"}, {"value": "0", "module": "C1"}, {"value": "0.107884462108115", "module": "C2"}, {"value": "0.774627080193552", "module": "C3"}, {"value": "0.0528112479418819", "module": "C4"}, {"value": "-0.775635142742623", "module": "D"}]}}, {"referenceToLCIAMethodDataSet": {"shortDescription": [{"value": "Global Warming Potential biogenic (GWP-biogenic)", "lang": "en"}, {"value": "Globales Erwärmungspotenzial biogen (GWP-biogenic)", "lang": "de"}], "type": "LCIA method data set", "refObjectId": "2356e1ab-0185-4db5-86e5-16de51c7485c", "uri": "../lciamethods/2356e1ab-0185-4db5-86e5-16de51c7485c.xml"}, "other": {"anies": [{"name": "referenceToUnitGroupDataSet", "value": {"shortDescription": [{"value": "kg CO_(2) eq", "lang": "en"}], "type": "unit group data set", "refObjectId": "1ebf3012-d0db-4de2-aefd-ef30cedb0be1", "uri": "../unitgroups/1ebf3012-d0db-4de2-aefd-ef30cedb0be1.xml"}}, {"value": "-0.251290469001783", "module": "A1"}, {"value": "-0.000554805705174584", "module": "A2"}, {"value": "-0.250899529119494", "module": "A3"}, {"value": "-0.000279535292410238", "module": "A4"}, {"value": "0.211504389515387", "module": "A5"}, {"value": "0", "module": "C1"}, {"value": "-0.000296287848466322", "module": "C2"}, {"value": "-2.69459864354067E-05", "module": "C3"}, {"value": "0.198510248835187", "module": "C4"}, {"value": "-0.0028484446806451", "module": "D"}]}}, {"referenceToLCIAMethodDataSet": {"shortDescription": [{"value": "Global Warming Potential luluc (GWP-luluc)", "lang": "en"}, {"value": "Globales Erwärmungspotenzial luluc (GWP-luluc)", "lang": "de"}], "type": "LCIA method data set", "refObjectId": "4331bbdb-978a-490d-8707-eeb047f01a55", "uri": "../lciamethods/4331bbdb-978a-490d-8707-eeb047f01a55.xml"}, "other": {"anies": [{"name": "referenceToUnitGroupDataSet", "value": {"shortDescription": [{"value": "kg CO_(2) eq", "lang": "en"}], "type": "unit group data set", "refObjectId": "1ebf3012-d0db-4de2-aefd-ef30cedb0be1", "uri": "../unitgroups/1ebf3012-d0db-4de2-aefd-ef30cedb0be1.xml"}}, {"value": "0.00773177623266228", "module": "A1"}, {"value": "0.00210767485707754", "module": "A2"}, {"value": "0.000585991325771231", "module": "A3"}, {"value": "0.000950629218256663", "module": "A4"}, {"value": "0.000189434594462578", "module": "A5"}, {"value": "0", "module": "C1"}, {"value": "0.00100760036103734", "module": "C2"}, {"value": "5.95353590673551E-05", "module": "C3"}, {"value": "0.000107166847690569", "module": "C4"}, {"value": "-0.00028785371271666", "module": "D"}]}}, {"referenceToLCIAMethodDataSet": {"shortDescription": [{"value": "Depletion potential of the stratospheric ozone layer (ODP)", "lang": "en"}, {"value": "Abbau Potential der stratosphärischen Ozonschicht (ODP)", "lang": "de"}], "type": "LCIA method data set", "refObjectId": "b5c629d6-def3-11e6-bf01-fe55135034f3", "uri": "../lciamethods/b5c629d6-def3-11e6-bf01-fe55135034f3.xml"}, "other": {"anies": [{"name": "referenceToUnitGroupDataSet", "value": {"shortDescription": [{"value": "kg CFC11 eq", "lang": "en"}], "type": "unit group data set", "refObjectId": "d9e957c9-7309-4474-bf3a-7777df6c4e5b", "uri": "../unitgroups/d9e957c9-7309-4474-bf3a-7777df6c4e5b.xml"}}, {"value": "7.52926930285951E-09", "module": "A1"}, {"value": "3.40424147886597E-14", "module": "A2"}, {"value": "1.0701815408331E-09", "module": "A3"}, {"value": "1.33557042395713E-14", "module": "A4"}, {"value": "1.3790642102667E-09", "module": "A5"}, {"value": "0", "module": "C1"}, {"value": "1.41561106636074E-14", "module": "C2"}, {"value": "9.74123684717578E-14", "module": "C3"}, {"value": "9.95056252673055E-14", "module": "C4"}, {"value": "-3.44107770673982E-12", "module": "D"}]}}, {"referenceToLCIAMethodDataSet": {"shortDescription": [{"value": "Acidification potential of land and water (AP)", "lang": "en"}, {"value": "Versauerungspotenzial von Boden und Wasser (AP)", "lang": "de"}], "type": "LCIA method data set", "refObjectId": "b5c611c6-def3-11e6-bf01-fe55135034f3", "uri": "../lciamethods/b5c611c6-def3-11e6-bf01-fe55135034f3.xml"}, "other": {"anies": [{"name": "referenceToUnitGroupDataSet", "value": {"shortDescription": [{"value": "mol H^(+) eq", "lang": "en"}], "type": "unit group data set", "refObjectId": "42e089ac-92bf-4bf2-8ca1-5fc40d18f2ed", "uri": "../unitgroups/42e089ac-92bf-4bf2-8ca1-5fc40d18f2ed.xml"}}, {"value": "0.0296157710803622", "module": "A1"}, {"value": "0.00109521822829556", "module": "A2"}, {"value": "0.00124223989563318", "module": "A3"}, {"value": "0.000148496249497425", "module": "A4"}, {"value": "9.34399419461773E-05", "module": "A5"}, {"value": "0", "module": "C1"}, {"value": "0.000179353164606158", "module": "C2"}, {"value": "0.000638772587200503", "module": "C3"}, {"value": "0.000283446337992513", "module": "C4"}, {"value": "-0.00126032818765095", "module": "D"}]}}, {"referenceToLCIAMethodDataSet": {"shortDescription": [{"value": "Eutrophication potential aquatic freshwater (EP-freshwater)", "lang": "en"}, {"value": "Eutrophierungspotenzial Süßwasser (EP-freshwater)", "lang": "de"}], "type": "LCIA method data set", "refObjectId": "b53ec18f-7377-4ad3-86eb-cc3f4f276b2b", "uri": "../lciamethods/b53ec18f-7377-4ad3-86eb-cc3f4f276b2b.xml"}, "other": {"anies": [{"name": "referenceToUnitGroupDataSet", "value": {"shortDescription": [{"value": "kg P eq", "lang": "en"}], "type": "unit group data set", "refObjectId": "0429039d-a61d-4590-ba67-aa4a20a810a1", "uri": "../unitgroups/0429039d-a61d-4590-ba67-aa4a20a810a1.xml"}}, {"value": "2.99240977406173E-05", "module": "A1"}, {"value": "8.53661534562517E-07", "module": "A2"}, {"value": "2.52687745039592E-05", "module": "A3"}, {"value": "3.75276855820526E-07", "module": "A4"}, {"value": "1.32956832382472E-06", "module": "A5"}, {"value": "0", "module": "C1"}, {"value": "3.97767171628871E-07", "module": "C2"}, {"value": "5.18174356730876E-08", "module": "C3"}, {"value": "2.36716363763868E-06", "module": "C4"}, {"value": "-3.96074273610254E-07", "module": "D"}]}}, {"referenceToLCIAMethodDataSet": {"shortDescription": [{"value": "Eutrophication potential aquatic marine (EP-marine)", "lang": "en"}, {"value": "Eutrophierungspotenzial Salzwasser (EP-marine)", "lang": "de"}], "type": "LCIA method data set", "refObjectId": "b5c619fa-def3-11e6-bf01-fe55135034f3", "uri": "../lciamethods/b5c619fa-def3-11e6-bf01-fe55135034f3.xml"}, "other": {"anies": [{"name": "referenceToUnitGroupDataSet", "value": {"shortDescription": [{"value": "kg N eq", "lang": "en"}], "type": "unit group data set", "refObjectId": "d05bb823-ecdf-4686-8c40-bf1d9257859f", "uri": "../unitgroups/d05bb823-ecdf-4686-8c40-bf1d9257859f.xml"}}, {"value": "0.00550584315766414", "module": "A1"}, {"value": "0.000447478390009414", "module": "A2"}, {"value": "0.00029182110691033", "module": "A3"}, {"value": "5.31444584874443E-05", "module": "A4"}, {"value": "3.51882169369881E-05", "module": "A5"}, {"value": "0", "module": "C1"}, {"value": "6.80728577209063E-05", "module": "C2"}, {"value": "0.000314761394727111", "module": "C3"}, {"value": "0.000177873818561136", "module": "C4"}, {"value": "-0.000350522972265309", "module": "D"}]}}, {"referenceToLCIAMethodDataSet": {"shortDescription": [{"value": "Eutrophication potential terrestrial (EP-terrestrial)", "lang": "en"}, {"value": "Eutrophierungspotenzial Land (EP-terrestrial)", "lang": "de"}], "type": "LCIA method data set", "refObjectId": "b5c614d2-def3-11e6-bf01-fe55135034f3", "uri": "../lciamethods/b5c614d2-def3-11e6-bf01-fe55135034f3.xml"}, "other": {"anies": [{"name": "referenceToUnitGroupDataSet", "value": {"shortDescription": [{"value": "mol N eq", "lang": "en"}], "type": "unit group data set", "refObjectId": "71b4d617-0ec9-4d3f-b65e-e438940c2401", "uri": "../unitgroups/71b4d617-0ec9-4d3f-b65e-e438940c2401.xml"}}, {"value": "0.118647411085306", "module": "A1"}, {"value": "0.00500854352174871", "module": "A2"}, {"value": "0.00277612002794457", "module": "A3"}, {"value": "0.000632906832177492", "module": "A4"}, {"value": "0.000366849882207106", "module": "A5"}, {"value": "0", "module": "C1"}, {"value": "0.000797786120648431", "module": "C2"}, {"value": "0.00356025978811276", "module": "C3"}, {"value": "0.000855321450964659", "module": "C4"}, {"value": "-0.00378556656389443", "module": "D"}]}}, {"referenceToLCIAMethodDataSet": {"shortDescription": [{"value": "Formation potential of tropospheric ozone photochemical oxidants (POCP)", "lang": "en"}, {"value": "Bildungspotential für troposphärisches Ozon (POCP)", "lang": "de"}], "type": "LCIA method data set", "refObjectId": "b5c610fe-def3-11e6-bf01-fe55135034f3", "uri": "../lciamethods/b5c610fe-def3-11e6-bf01-fe55135034f3.xml"}, "other": {"anies": [{"name": "referenceToUnitGroupDataSet", "value": {"shortDescription": [{"value": "kg NMVOC eq", "lang": "en"}], "type": "unit group data set", "refObjectId": "d27c25f8-fbc1-44c6-b47b-4adbae4199c6", "uri": "../unitgroups/d27c25f8-fbc1-44c6-b47b-4adbae4199c6.xml"}}, {"value": "0.0139813517240635", "module": "A1"}, {"value": "0.00119892453777315", "module": "A2"}, {"value": "0.000699362175295405", "module": "A3"}, {"value": "0.000129290486988935", "module": "A4"}, {"value": "0.000100564972625371", "module": "A5"}, {"value": "0", "module": "C1"}, {"value": "0.000159893745126605", "module": "C2"}, {"value": "0.000809217928930353", "module": "C3"}, {"value": "0.000305313209923271", "module": "C4"}, {"value": "-0.00109813764612559", "module": "D"}]}}, {"referenceToLCIAMethodDataSet": {"shortDescription": [{"value": "Abiotic depletion potential for non fossil resources (ADPE)", "lang": "en"}, {"value": "Potenzial für den abiotischen Abbau nicht fossiler Ressourcen (ADPE)", "lang": "de"}], "type": "LCIA method data set", "refObjectId": "b2ad6494-c78d-11e6-9d9d-cec0c932ce01", "uri": "../lciamethods/b2ad6494-c78d-11e6-9d9d-cec0c932ce01.xml"}, "other": {"anies": [{"name": "referenceToUnitGroupDataSet", "value": {"shortDescription": [{"value": "kg Sb eq", "lang": "en"}], "type": "unit group data set", "refObjectId": "54ccd2d9-a32a-4fc2-923d-f2c8c93e89d4", "uri": "../unitgroups/54ccd2d9-a32a-4fc2-923d-f2c8c93e89d4.xml"}}, {"value": "1.17635878732494E-05", "module": "A1"}, {"value": "1.73888392174141E-08", "module": "A2"}, {"value": "6.83722317235903E-07", "module": "A3"}, {"value": "6.80534202158474E-09", "module": "A4"}, {"value": "5.9997448223454E-08", "module": "A5"}, {"value": "0", "module": "C1"}, {"value": "7.21318569453014E-09", "module": "C2"}, {"value": "8.68103845937878E-09", "module": "C3"}, {"value": "1.76058245385473E-09", "module": "C4"}, {"value": "-4.57247481458976E-08", "module": "D"}]}}, {"referenceToLCIAMethodDataSet": {"shortDescription": [{"value": "Abiotic depletion potential for fossil resources (ADPF)", "lang": "en"}, {"value": "Potenzial für den abiotischen Abbau fossiler Brennstoffe (ADPF)", "lang": "de"}], "type": "LCIA method data set", "refObjectId": "b2ad6110-c78d-11e6-9d9d-cec0c932ce01", "uri": "../lciamethods/b2ad6110-c78d-11e6-9d9d-cec0c932ce01.xml"}, "other": {"anies": [{"name": "referenceToUnitGroupDataSet", "value": {"shortDescription": [{"value": "MJ", "lang": "en"}], "type": "unit group data set", "refObjectId": "93a60a57-a3c8-11da-a746-0800200c9a66", "uri": "../unitgroups/93a60a57-a3c8-11da-a746-0800200c9a66.xml"}}, {"value": "127.855838690163", "module": "A1"}, {"value": "3.64816864256112", "module": "A2"}, {"value": "3.99734737514888", "module": "A3"}, {"value": "1.3982643195799", "module": "A4"}, {"value": "0.56055385246986", "module": "A5"}, {"value": "0", "module": "C1"}, {"value": "1.48206220277772", "module": "C2"}, {"value": "0.400606111261862", "module": "C3"}, {"value": "0.592451751022522", "module": "C4"}, {"value": "-11.5026330699804", "module": "D"}]}}, {"referenceToLCIAMethodDataSet": {"shortDescription": [{"value": "Water use (WDP)", "lang": "en"}, {"value": "Wassernutzung (WDP)", "lang": "de"}], "type": "LCIA method data set", "refObjectId": "b2ad66ce-c78d-11e6-9d9d-cec0c932ce01", "uri": "../lciamethods/b2ad66ce-c78d-11e6-9d9d-cec0c932ce01.xml"}, "other": {"anies": [{"name": "referenceToUnitGroupDataSet", "value": {"shortDescription": [{"value": "m^(3) world eq deprived", "lang": "en"}], "type": "unit group data set", "refObjectId": "6ae2df01-888e-46c8-b17d-49fa3869b476", "uri": "../unitgroups/6ae2df01-888e-46c8-b17d-49fa3869b476.xml"}}, {"value": "0.972430669355923", "module": "A1"}, {"value": "0.00308238735181487", "module": "A2"}, {"value": "0.074590314019698", "module": "A3"}, {"value": "0.00124032256438218", "module": "A4"}, {"value": "0.00215779491506429", "module": "A5"}, {"value": "0", "module": "C1"}, {"value": "0.0013146550092013", "module": "C2"}, {"value": "0.0998567649188251", "module": "C3"}, {"value": "0.0043062505120456", "module": "C4"}, {"value": "-0.0167117443725716", "module": "D"}]}}, {"referenceToLCIAMethodDataSet": {"shortDescription": [{"value": "Incidence of disease due to PM emissions (PM)", "lang": "en"}, {"value": "Auftreten von Krankheiten aufgrund von Feinstaubemissionen (PM)", "lang": "de"}], "type": "LCIA method data set", "refObjectId": "b5c602c6-def3-11e6-bf01-fe55135034f3", "uri": "../lciamethods/b5c602c6-def3-11e6-bf01-fe55135034f3.xml"}, "other": {"anies": [{"name": "referenceToUnitGroupDataSet", "value": {"shortDescription": [{"value": "Disease incidence", "lang": "en"}], "type": "unit group data set", "refObjectId": "3883559b-648f-4afc-8ba2-0bd24f3affa3", "uri": "../unitgroups/3883559b-648f-4afc-8ba2-0bd24f3affa3.xml"}}, {"value": "3.17362654237489E-07", "module": "A1"}, {"value": "2.25212605569281E-08", "module": "A2"}, {"value": "1.41393740613457E-08", "module": "A3"}, {"value": "1.29055918761629E-09", "module": "A4"}, {"value": "1.22505240821533E-09", "module": "A5"}, {"value": "0", "module": "C1"}, {"value": "1.2168058266724E-09", "module": "C2"}, {"value": "2.92346187606402E-09", "module": "C3"}, {"value": "3.32104685617553E-09", "module": "C4"}, {"value": "-1.59478787647649E-08", "module": "D"}]}}, {"referenceToLCIAMethodDataSet": {"shortDescription": [{"value": "Human exposure efficiency relative to U235 (IR)", "lang": "en"}, {"value": "Wirkung durch Exposition des Menschen mit U235 (IR)", "lang": "de"}], "type": "LCIA method data set", "refObjectId": "b5c632be-def3-11e6-bf01-fe55135034f3", "uri": "../lciamethods/b5c632be-def3-11e6-bf01-fe55135034f3.xml"}, "other": {"anies": [{"name": "referenceToUnitGroupDataSet", "value": {"shortDescription": [{"value": "kBq U235 eq", "lang": "en"}], "type": "unit group data set", "refObjectId": "456b05bf-1415-44a9-9993-02452f554c09", "uri": "../unitgroups/456b05bf-1415-44a9-9993-02452f554c09.xml"}}, {"value": "0.537637745283801", "module": "A1"}, {"value": "0.000993257635089982", "module": "A2"}, {"value": "0.016870898790852", "module": "A3"}, {"value": "0.000391704557387109", "module": "A4"}, {"value": "0.00338771768493001", "module": "A5"}, {"value": "0", "module": "C1"}, {"value": "0.000415179384205146", "module": "C2"}, {"value": "0.00180052446773737", "module": "C3"}, {"value": "0.000856861966828969", "module": "C4"}, {"value": "-0.0499306752116612", "module": "D"}]}}, {"referenceToLCIAMethodDataSet": {"shortDescription": [{"value": "Comparative toxic unit for ecosystems (ETP-fw)", "lang": "en"}, {"value": "Toxizitätsvergleichseinheit für Ökosysteme (ETP-fw)", "lang": "de"}], "type": "LCIA method data set", "refObjectId": "ee1082d1-b0f7-43ca-a1f0-21e2a4a74511", "uri": "../lciamethods/ee1082d1-b0f7-43ca-a1f0-21e2a4a74511.xml"}, "other": {"anies": [{"name": "referenceToUnitGroupDataSet", "value": {"shortDescription": [{"value": "CTUe", "lang": "en"}], "type": "unit group data set", "refObjectId": "aa959ded-f1eb-4efb-9c5c-2d60be36b3e6", "uri": "../unitgroups/aa959ded-f1eb-4efb-9c5c-2d60be36b3e6.xml"}}, {"value": "171.233493147679", "module": "A1"}, {"value": "2.67069805835496", "module": "A2"}, {"value": "2.02951986209959", "module": "A3"}, {"value": "1.00167223395983", "module": "A4"}, {"value": "0.258669449138542", "module": "A5"}, {"value": "0", "module": "C1"}, {"value": "1.06168966710626", "module": "C2"}, {"value": "0.205556634416356", "module": "C3"}, {"value": "0.632049900359924", "module": "C4"}, {"value": "-2.63629098741354", "module": "D"}]}}, {"referenceToLCIAMethodDataSet": {"shortDescription": [{"value": "Comparative toxic unit for humans (carcinogenic) (HTP-c)", "lang": "en"}, {"value": "Toxizitätsvergleichseinheit für Menschen (krebserregend) (HTP-c)", "lang": "de"}], "type": "LCIA method data set", "refObjectId": "2299222a-bbd8-474f-9d4f-4dd1f18aea7c", "uri": "../lciamethods/2299222a-bbd8-474f-9d4f-4dd1f18aea7c.xml"}, "other": {"anies": [{"name": "referenceToUnitGroupDataSet", "value": {"shortDescription": [{"value": "CTUh", "lang": "en"}], "type": "unit group data set", "refObjectId": "d4c9523e-2d7e-49fd-8469-998f547d3a70", "uri": "../unitgroups/d4c9523e-2d7e-49fd-8469-998f547d3a70.xml"}}, {"value": "5.22911798403473E-09", "module": "A1"}, {"value": "5.20755906829683E-11", "module": "A2"}, {"value": "2.94824340358051E-10", "module": "A3"}, {"value": "2.03216642293446E-11", "module": "A4"}, {"value": "1.39898288478113E-11", "module": "A5"}, {"value": "0", "module": "C1"}, {"value": "2.15425590767326E-11", "module": "C2"}, {"value": "8.13159078596676E-12", "module": "C3"}, {"value": "4.3461178107282E-11", "module": "C4"}, {"value": "-6.35391665578662E-10", "module": "D"}]}}, {"referenceToLCIAMethodDataSet": {"shortDescription": [{"value": "Comparative toxic unit for humans (noncarcinogenic) (HTP-nc)", "lang": "en"}, {"value": "Toxizitätsvergleichseinheit für Menschen (nicht krebserregend) (HTP-nc)", "lang": "de"}], "type": "LCIA method data set", "refObjectId": "3af763a5-b7a1-48c9-9cee-1f223481fcef", "uri": "../lciamethods/3af763a5-b7a1-48c9-9cee-1f223481fcef.xml"}, "other": {"anies": [{"name": "referenceToUnitGroupDataSet", "value": {"shortDescription": [{"value": "CTUh", "lang": "en"}], "type": "unit group data set", "refObjectId": "d4c9523e-2d7e-49fd-8469-998f547d3a70", "uri": "../unitgroups/d4c9523e-2d7e-49fd-8469-998f547d3a70.xml"}}, {"value": "1.33649668610219E-07", "module": "A1"}, {"value": "2.15103871493408E-09", "module": "A2"}, {"value": "1.6698505245921E-09", "module": "A3"}, {"value": "9.04175881474677E-10", "module": "A4"}, {"value": "2.93211745400687E-10", "module": "A5"}, {"value": "0", "module": "C1"}, {"value": "9.58425278547678E-10", "module": "C2"}, {"value": "5.93433545721562E-10", "module": "C3"}, {"value": "4.58506212848425E-09", "module": "C4"}, {"value": "-2.20858008189758E-09", "module": "D"}]}}, {"referenceToLCIAMethodDataSet": {"shortDescription": [{"value": "Soil quality index (SQP)", "lang": "en"}, {"value": "Bodenqualitätsindex (SQP)", "lang": "de"}], "type": "LCIA method data set", "refObjectId": "b2ad6890-c78d-11e6-9d9d-cec0c932ce01", "uri": "../lciamethods/b2ad6890-c78d-11e6-9d9d-cec0c932ce01.xml"}, "other": {"anies": [{"name": "referenceToUnitGroupDataSet", "value": {"shortDescription": [{"value": "SQP", "lang": "en"}], "type": "unit group data set", "refObjectId": "f130951c-e67f-4f7f-8dd4-665de3974e18", "uri": "../unitgroups/f130951c-e67f-4f7f-8dd4-665de3974e18.xml"}}, {"value": "69.3980615998527", "module": "A1"}, {"value": "1.30152642876316", "module": "A2"}, {"value": "7.23882178448549", "module": "A3"}, {"value": "0.584251128328543", "module": "A4"}, {"value": "0.194356562480014", "module": "A5"}, {"value": "0", "module": "C1"}, {"value": "0.619265257720461", "module": "C2"}, {"value": "0.0944062136885545", "module": "C3"}, {"value": "0.116652651325226", "module": "C4"}, {"value": "-1.8272079029651", "module": "D"}]}}]}, "otherAttributes": {"{http://www.indata.network/EPD/2019}epd-version": "1.2"}, "version": "1.1", "locations": "../ILCDLocations.xml"}