{"processInformation": {"dataSetInformation": {"UUID": "127a23f5-d954-41c9-8f8a-ecca18aca691", "name": {"baseName": [{"value": "Vormauerziegel und Klinker", "lang": "de"}, {"value": "Facing bricks", "lang": "en"}], "functionalUnitFlowProperties": [{"lang": "de"}]}, "classificationInformation": {"classification": [{"class": [{"value": "Mineralische Baustoffe", "level": 0, "classId": "1"}, {"value": "Steine und Elemente", "level": 1, "classId": "1.3"}, {"value": "Ziegel", "level": 2, "classId": "1.3.02"}], "name": "OEKOBAU.DAT"}, {"class": [{"value": "02 Bauprodukte", "level": 0}, {"value": "Mauerwerk und Mörtel", "level": 1}, {"value": "Ziegel", "level": 2}], "name": "IBUCategories"}]}, "generalComment": [{"value": "Vormauerziegel und Klinker gehren zur Gruppe der grobkeramischen gebrannten Tonbaustoffe.\nAuf Basis der massenbezogenen Jahresproduktion wurden die Anteile der einzelnen Firmen an der Gesamtproduktion ermittelt und zur Berechnung der gewichteten Durchschnittswerte verwendet. In dieser EPD erfolgt die Darstellung der kobilanzergebnisse der Vormauerziegel und Klinker fr einen Quadratmeter (1 m).", "lang": "de"}, {"value": "Facing bricks belong to the group of heavy-clay building materials. \nBased on mass-related annual production, the shares contributed to overall production by the individual companies were identified and used to calculate the weighted average values. This EPD presents the LCA results for one square metre (1 m) each of facing bricks.", "lang": "en"}], "other": {"anies": [{"scenario": [{"description": [{"value": "Gutschriften infolge des Recyclings der Bauschuttaufbereitung Im End of Life der Vormauerziegel und Klinker wird im Rahmen dieses Wiederverwertungsszenarios eine Materialgutschrift für Kies angesetzt.", "lang": "de"}, {"value": "Credits resulting from the recycling of construction waste processing In the end-of-life of facing bricks and clinker, a material credit for gravel is recognized as part of this recycling scenario.", "lang": "en"}], "name": "S0", "default": true}, {"description": [{"value": "Gutschriften infolge der thermischen Verwertung der Verpackungsmaterialien (aus Modul A5) werden in Modul D/1 ausgewiesen.", "lang": "de"}, {"value": "Credits resulting from the thermal recycling of packaging materials (from module A5) are reported in module D/1.", "lang": "en"}], "name": "S1"}]}]}}, "quantitativeReference": {"referenceToReferenceFlow": [0]}, "time": {"referenceYear": 2023, "dataSetValidUntil": 2028, "other": {"anies": [{"name": "publicationDateOfEPD", "value": 1679270400000}]}}, "geography": {"locationOfOperationSupplyOrProduction": {"location": "DE"}}, "technology": {"technologyDescriptionAndIncludedProcesses": [{"value": "Grubenbetrieb Die Hauptbestandteile (Lehm und Ton) werden im Tagebaubetrieb abgebaut. Der Abbau erfolgt nach Abziehen des Oberbodens und ggf. Bearbeitung von archäologischen Fundstellen in der Regel mit Löffelbaggern. Der Transport wird je nach Straßenverhältnissen mit geeigneten Lkw durchgeführt. Bei kurzen Entfernungen können Bandstraßen zum Einsatz kommen. Wenn die Gruben erschöpft sind, werden sie entsprechend den Vorgaben des Naturschutzes rekultiviert und ggf. der vorherigen Nutzung wieder zugeführt. Rohstoffaufbereitung Die einzelnen Rohstoffkomponenten werden beprobt und im Labor auf ihre keramischen Eigenschaften und ihre mineralogischen und chemischen Zusammensetzungen hin analysiert. In der Aufbereitung werden die Komponenten entsprechend ihrer keramischen Eigenschaften zur Betriebsmasse vereint, homogenisiert und gelagert. Formgebung Die Betriebsmasse wird stranggezogen und mit Hilfe von Abschneidern für die jeweiligen Formate geschnitten. Verschiedene Parameter wie Pressenvakuum, Feuchte und Plastizität werden regelmäßig kontrolliert. Überschüssige Betriebsmasse und fehlerhafte Pressungen werden vollständig in den Massekreislauf zurückgeführt. Trocknung Das Trocknen dient als Vorbereitung des plastischen Ziegels für den darauffolgenden Brennvorgang und erfolgt je nach Modell über 1 – 2 Tage bei ca. 60 – 120 °C. Aufgrund des Schwindungsverhalten reagiert das keramische Material sehr empfindlich und muss deshalb unter definierten Bedingungen getrocknet werden. Verschiedene Trocknungsparameter sowie die Restfeuchte werden ständig kontrolliert. Aussortierte getrocknete Ziegel (Trockenbruch) werden in der Rohstoffaufbereitung wieder der Betriebsmasse zugeführt. Brennen Die Ziegel werden in Tunnel und Herdwagenöfen (in seltenen Fällen auch in Ringöfen) unter Verwendung von Erdgas bei ca. 1000 – 1200 °C gebrannt. Die Brenndauer inkl. Aufheiz- und Abkühlphase beträgt ca. 1 – 2 Tage. Durch den Brand erhalten die Ziegel ihre keramischen Eigenschaften, die sie langlebig und beständig machen. Qualitätskontrolle Die geforderten keramischen Qualitätseigenschaften nach EN 771-1 und die einzuhaltenden Produktmaße werden in der werkseigenen Produktionskontrolle (WPK) regelmäßig intern kontrolliert und zusätzlich mindestens jährlich extern überwacht \nTechnische Daten: \nBautechnische Daten\nAlle relevanten bautechnischen Daten sind in der nachfolgenden Tabelle aufgelistet. Alle weiteren bautechnischen Daten gem PCR: Ziegel wurden nicht aufgelistet, da\ndiese fr das deklarierte Produkt in der Praxis irrelevant bzw. nicht den\nbautechnischen Eigenschaften entsprechen. \nDeklarierte Einheit: \nDie Deklaration bezieht sich auf 1 m2 Wand aus Vormauerziegeln und Klinkern (Maße des Steins (mm): 240 x 115 x 71, Mörtelfuge: 12, ohne Mörtel).", "lang": "de"}, {"value": "Pit operation The main components (loam and clay) are extracted in opencast mines. After the topsoil has been removed and, if necessary, archaeological sites have been processed, extraction is usually carried out with excavators. Depending on the road conditions, transport entails the use of suitable trucks. Conveyor belts can be used for short distances. When the pits are exhausted, they are recultivated in accordance with nature conservation guidelines and, if necessary, returned to their previous use. Processing raw materials The individual raw material components are sampled and analysed in the laboratory for their ceramic properties and their mineralogical and chemical compositions. In the processing stage, the components are combined into the operating mass according to their ceramic properties, homogenised and stored. Forming The production mass is extruded and cut to the respective formats using cutters. Various parameters such as press vacuum, moisture and plasticity are checked regularly. Excess operating mass and faulty pressings are returned in full to the mass circuit. Drying Drying serves as preparation of the plastic tile for the subsequent firing process and takes place over 1–2 days at approx. 60–120 °C, depending on the model. Due to its shrinkage behaviour, the ceramic material reacts very sensitively and must therefore be dried under defined conditions. Various drying parameters and the residual moisture are constantly monitored. Dried bricks that have been sorted out (dry quarry) are returned to the production mass in the raw material preparation department. Firing The bricks are fired in tunnel kilns and bogie hearth furnaces (also in ring furnaces in rare cases) at approx. 1000–1200 °C using natural gas. The firing time incl. the heating and cooling phase is approx. 1–2 days. The firing process gives the bricks their ceramic properties, which make them durable and long-lasting. Quality control The requisite ceramic quality properties according to EN 771­1 and the product dimensions to be adhered to are regularly controlled internally in the factory's own production control and additionally monitored externally at least once a year. \nTechnical data: \nStructural data \nAll relevant structural data is listed in the following table. All other structural data in accordance with the PCR. Bricks are not listed as they are not of relevance in practice for the declared product or do not comply with the structural data. \nDeclared unit: \nThe Declaration refers to 1 m wall comprising facing bricks (brick size (mm): 240 x 115 x 71, mortar joint: 12, without mortar).", "lang": "en"}], "technologicalApplicability": [{"value": "Vormauerziegel werden als Sichtmauerwerk in zweischaligen Wandkonstruktionen im vor der Witterung ungeschützten Außenbereich oder als Sichtmauerwerk im Innenbereich verwendet.", "lang": "de"}, {"value": "Facing bricks are used as exposed brickwork in double wall constructions in exterior areas not protected from weathering or as exposed brickwork in indoor applications.", "lang": "en"}], "referenceToTechnologyFlowDiagrammOrPicture": [{"shortDescription": [{"value": "Bautechnsiche Daten VMZjpg.jpg", "lang": "de"}], "type": "source data set", "refObjectId": "a8bd4343-78a9-4482-9b64-d2d3c3cfbbbb", "uri": "../sources/a8bd4343-78a9-4482-9b64-d2d3c3cfbbbb.xml"}]}}, "modellingAndValidation": {"LCIMethodAndAllocation": {"typeOfDataSet": "EPD", "referenceToLCAMethodDetails": [{"shortDescription": [{"value": "Ziegel.pdf", "lang": "de"}], "type": "source data set", "refObjectId": "2bfc0ec4-792f-4892-a451-ca8b0c6143c3"}], "other": {"anies": [{"name": "subType", "value": "average dataset"}]}}, "dataSourcesTreatmentAndRepresentativeness": {"referenceToDataSource": [{"shortDescription": [{"value": "GaBi Database (all versions)", "lang": "de"}], "type": "source data set", "refObjectId": "28d74cc0-db8b-4d7e-bc44-5f6d56ce0c4a"}, {"shortDescription": [{"value": "GaBi Database Edition 2022, CUP 2022.02", "lang": "de"}], "type": "source data set", "refObjectId": "94f442cb-662e-43ea-a792-4b0a35132e93"}], "useAdviceForDataSet": [{"value": "Gültigkeitsbereich: \nDie Anwendung dieses Dokumentes ist auf Vormauerziegel und Klinker beschrnkt, die von Mitgliedsunternehmen des Bundesverbandes der Deutschen Ziegelindustrie e.V. hergestellt werden. Fr diese Deklaration wurden von 11 Mitgliedsunternehmen und insgesamt 11 Produktionsstandorten Daten aus dem Jahr 2021 zur Verfgung gestellt.\nDiese Mitglieder reprsentieren nach Anzahl rund 90 % der im Bundesverband zusammengeschlossenen Hersteller von Vormauerziegeln und Klinker. Das Produktionsvolumen dieser Firmen liegt nach Produktionsmenge bei ca. 90 % des deutschen Marktes. \nSystemgrenze: \nTyp der EPD: Wiege bis zum Werkstor- mit Optionen. Die kobilanz bercksichtigt die Rohstoffgewinnung, die Rohstofftransporte und die eigentliche Produktherstellung inklusive der Verpackungsmaterialien (Module A1–A3). Der Transport zur Baustelle (Modul A4) sowie die Behandlung der Verpackungsmaterialien in Mllverbrennungsanlagen nach dem Einbau des Produktes (Modul A5) sind ebenfalls Teil der Systemgrenzen. Nach Ablauf der Nutzungsdauer wird das Produkt mit Hilfe eines Baggers rckgebaut (Modul C1). Nach dem Transport des rckgebauten Produktes (Modul C2) ist fr rund 6 % der Vormauerziegel und Klinker eine Deponierung auf einer Inertstoffdeponie vorgesehen (Modul C4), 94 % knnen nach der Aufbereitung (Modul C3) weiterverwertet werden. Gutschriften infolge des Recyclings von Ziegelbruch sind in Modul D deklariert. Gutschriften fr Strom und thermische Energie infolge der thermischen Verwertung der Verpackung innerhalb des Moduls A5 werden ebenfalls in Modul D/1 bercksichtigt.", "lang": "de"}, {"value": "Scope: \nApplication of this document is restricted to facing bricks manufactured by member companies of the Bundesverband der Deutschen Ziegelindustrie e.V. For this Declaration, data from 2021 was made available by 11 member companies and a total of 11 production locations. These members represent around 90% of the manufacturers of facing bricks united in the federal association. Depending on their respective production quantities, the production volume of these companies accounts for approx. 90% of the German market. \nSystem boundary: \nType of EPD: cradle to plant gate – with options. The Life Cycle Assessment takes into account the extraction of raw materials, the transport of raw materials and actual product manufacturing, including packaging materials (Modules A1–A3). Transport to the construction site (Module A4) and treatment of the packaging materials in the waste incineration plants following installation of the product (Module A5) are also part of the system boundaries. At the end of its useful life, the product is deconstructed using a digger (Module C1). After transport of the deconstructed product (Module C2), about 6 % of the facing bricks are to be disposed of in an inert waste landfill (Module C4), 94 % can be reused after processing (Module C3). \nCredits incurred by recycling firing waste are declared in Module D. Credits for electricity and thermal energy following thermal utilisation of packaging within Module A5 are also considered in Module D/1.", "lang": "en"}], "other": {"anies": [{"name": "referenceToOriginalEPD", "value": {"shortDescription": {"value": "Vormauerziegel und Klinker.pdf", "defaultValue": "Vormauerziegel und Klinker.pdf", "lstrings": [{"lang": "de", "value": "Vormauerziegel und Klinker.pdf"}]}, "type": "source data set", "uuid": {"uuid": "230ef271-f516-405f-826c-fd47a85ec73c"}, "refObjectId": "230ef271-f516-405f-826c-fd47a85ec73c", "resourceURLs": ["https://oekobaudat.de/OEKOBAU.DAT/resource/sources/230ef271-f516-405f-826c-fd47a85ec73c/Vormauerziegel_und_Klinker_18526.pdf?version=00.02.000"]}}]}}, "validation": {"review": [{"referenceToNameOfReviewerAndInstitution": [{"shortDescription": [{"value": "Institut Bauen und Umwelt e. V.", "lang": "de"}], "type": "contact data set", "refObjectId": "d111dbec-b024-4be5-86c5-752d6eb2cf95", "uri": "../contacts/d111dbec-b024-4be5-86c5-752d6eb2cf95.xml"}], "type": "Accredited third party review"}]}, "complianceDeclarations": {"compliance": [{"referenceToComplianceSystem": {"shortDescription": [{"value": "DIN EN 15804+A2", "lang": "de"}], "type": "source data set", "refObjectId": "c0016b33-8cf7-415c-ac6e-deba0d21440d", "uri": "../sources/c0016b33-8cf7-415c-ac6e-deba0d21440d.xml"}}, {"referenceToComplianceSystem": {"shortDescription": [{"value": "ISO 14025", "lang": "de"}], "type": "source data set", "refObjectId": "4f2eb655-6e44-4874-a95a-e28f5442cd4d", "uri": "../sources/4f2eb655-6e44-4874-a95a-e28f5442cd4d.xml"}}]}}, "administrativeInformation": {"commissionerAndGoal": {"referenceToCommissioner": [{"shortDescription": [{"value": "Bundesverband der Deutschen Ziegelindustrie e.V.", "lang": "de"}], "type": "contact data set", "refObjectId": "44c3c786-9704-4e55-9729-ab211a1916fb", "uri": "../contacts/44c3c786-9704-4e55-9729-ab211a1916fb.xml"}]}, "dataGenerator": {"referenceToPersonOrEntityGeneratingTheDataSet": [{"shortDescription": [{"value": "Life Cycle Engineering Experts GmbH", "lang": "de"}], "type": "contact data set", "refObjectId": "2eed094a-ec91-42be-9e41-01ae55b495b9", "uri": "../contacts/2eed094a-ec91-42be-9e41-01ae55b495b9.xml"}]}, "dataEntryBy": {"timeStamp": 1679270400000, "referenceToDataSetFormat": [{"shortDescription": [{"value": "ILCD Format", "lang": "de"}], "type": "source data set", "refObjectId": "a97a0155-0234-4b87-b4ce-a45da52f2a40", "uri": "../sources/a97a0155-0234-4b87-b4ce-a45da52f2a40.xml"}, {"shortDescription": [{"value": "EPD-Datenformaterweiterungen v1.2", "lang": "de"}, {"value": "EPD Data Format Extensions v1.2", "lang": "en"}], "type": "source data set", "refObjectId": "a29449fd-aa2f-4de8-b5d7-4b06b43c6fde", "uri": "../sources/a29449fd-aa2f-4de8-b5d7-4b06b43c6fde.xml"}]}, "publicationAndOwnership": {"dataSetVersion": "00.12.000", "referenceToRegistrationAuthority": {"shortDescription": [{"value": "Institut Bauen und Umwelt e. V.", "lang": "de"}], "type": "contact data set", "refObjectId": "d111dbec-b024-4be5-86c5-752d6eb2cf95", "uri": "../contacts/d111dbec-b024-4be5-86c5-752d6eb2cf95.xml"}, "registrationNumber": "EPD-BDZ-20230091-ICG1-DE", "referenceToOwnershipOfDataSet": {"shortDescription": [{"value": "Bundesverband der Deutschen Ziegelindustrie e.V.", "lang": "de"}], "type": "contact data set", "refObjectId": "44c3c786-9704-4e55-9729-ab211a1916fb", "uri": "../contacts/44c3c786-9704-4e55-9729-ab211a1916fb.xml"}, "copyright": true, "licenseType": "Free of charge for all users and uses", "accessRestrictions": [{"value": "None", "lang": "en"}], "other": {"anies": [{"name": "referenceToPublisher", "value": {"shortDescription": [{"value": "Institut Bauen und Umwelt e. V.", "lang": "de"}], "type": "contact data set", "refObjectId": "d111dbec-b024-4be5-86c5-752d6eb2cf95", "uri": "../contacts/d111dbec-b024-4be5-86c5-752d6eb2cf95.xml"}}]}}}, "exchanges": {"exchange": [{"dataSetInternalID": 0, "referenceToFlowDataSet": {"shortDescription": [{"value": "1 m² Vormauerziegel und Klinker (1 m² Vormauerziegel und Klinker)", "lang": "de"}], "type": "flow data set", "refObjectId": "a2bc00f1-b1c2-fa71-8f06-92f2a067d14b", "uri": "../flows/a2bc00f1-b1c2-fa71-8f06-92f2a067d14b.xml"}, "meanAmount": 1.0, "referencesToDataSource": {}, "referenceFlow": true, "resolvedFlowVersion": "00.06.000", "resultingflowAmount": 1.0, "flowProperties": [{"name": [{"lang": "en", "value": "Area"}, {"lang": "de", "value": "Fläche"}], "uuid": "93a60a56-a3c8-19da-a746-0800200c9a66", "referenceFlowProperty": true, "meanValue": 1.0, "referenceUnit": "qm", "unitGroupUUID": "c20a03d7-bd90-4569-bc94-66cfd364dfc8"}], "materialProperties": [{"name": "grammage", "value": "159.0", "unit": "kg/m^2", "unitDescription": "kilograms per square meter"}, {"name": "gross density", "value": "1700.0", "unit": "kg/m^3", "unitDescription": "kilograms per cubic metre"}, {"name": "layer thickness", "value": "0.071", "unit": "m", "unitDescription": "meters"}], "typeOfFlow": "Product flow", "classification": {"classHierarchy": "Mineralische Baustoffe / Steine und Elemente / Ziegel", "name": "OEKOBAU.DAT"}}, {"dataSetInternalID": 1, "referenceToFlowDataSet": {"shortDescription": [{"value": "Erneuerbare Primärenergie als Energieträger (PERE)", "lang": "de"}, {"value": "Renewable primary energy as energy carrier (PERE)", "lang": "en"}], "type": "flow data set", "refObjectId": "20f32be5-0398-4288-9b6d-accddd195317", "uri": "../flows/20f32be5-0398-4288-9b6d-accddd195317.xml"}, "exchange direction": "INPUT", "other": {"anies": [{"name": "referenceToUnitGroupDataSet", "value": {"shortDescription": [{"value": "MJ", "lang": "de"}], "type": "unit group data set", "refObjectId": "93a60a57-a3c8-11da-a746-0800200c9a66", "uri": "../unitgroups/93a60a57-a3c8-11da-a746-0800200c9a66.xml"}}, {"value": "36.291", "module": "A1-A3"}, {"value": "1.19", "module": "A4"}, {"value": "1.45", "module": "A5"}, {"value": "0.0769", "module": "C1"}, {"value": "0.206", "module": "C2"}, {"value": "0.605", "module": "C3"}, {"value": "0.286", "module": "C4"}, {"value": "-1.45", "module": "D", "scenario": "S0"}, {"value": "-1.4", "module": "D", "scenario": "S1"}]}, "resolvedFlowVersion": "38.00.000", "flowProperties": [], "typeOfFlow": "Other flow", "classification": {"classHierarchy": "Quantities", "name": "GaBiCategories"}}, {"dataSetInternalID": 2, "referenceToFlowDataSet": {"shortDescription": [{"value": "Erneuerbare Primärenergie zur stofflichen Nutzung (PERM)", "lang": "de"}, {"value": "Renewable primary energy resources as material utilization (PERM)", "lang": "en"}], "type": "flow data set", "refObjectId": "fb3ec0de-548d-4508-aea5-00b73bf6f702", "uri": "../flows/fb3ec0de-548d-4508-aea5-00b73bf6f702.xml"}, "exchange direction": "INPUT", "other": {"anies": [{"name": "referenceToUnitGroupDataSet", "value": {"shortDescription": [{"value": "MJ", "lang": "de"}], "type": "unit group data set", "refObjectId": "93a60a57-a3c8-11da-a746-0800200c9a66", "uri": "../unitgroups/93a60a57-a3c8-11da-a746-0800200c9a66.xml"}}, {"value": "1.44", "module": "A1-A3"}, {"value": "0", "module": "A4"}, {"value": "-1.44", "module": "A5"}, {"value": "0", "module": "C1"}, {"value": "0", "module": "C2"}, {"value": "0", "module": "C3"}, {"value": "0", "module": "C4"}, {"value": "0", "module": "D", "scenario": "S0"}, {"value": "0", "module": "D", "scenario": "S1"}]}, "resolvedFlowVersion": "38.00.000", "flowProperties": [], "typeOfFlow": "Other flow", "classification": {"classHierarchy": "Quantities", "name": "GaBiCategories"}}, {"dataSetInternalID": 3, "referenceToFlowDataSet": {"shortDescription": [{"value": "Total erneuerbare Primärenergie (PERT)", "lang": "de"}, {"value": "Total use of renewable primary energy resources (PERT)", "lang": "en"}], "type": "flow data set", "refObjectId": "53f97275-fa8a-4cdd-9024-65936002acd0", "uri": "../flows/53f97275-fa8a-4cdd-9024-65936002acd0.xml"}, "exchange direction": "INPUT", "other": {"anies": [{"name": "referenceToUnitGroupDataSet", "value": {"shortDescription": [{"value": "MJ", "lang": "de"}], "type": "unit group data set", "refObjectId": "93a60a57-a3c8-11da-a746-0800200c9a66", "uri": "../unitgroups/93a60a57-a3c8-11da-a746-0800200c9a66.xml"}}, {"value": "37.73", "module": "A1-A3"}, {"value": "1.19", "module": "A4"}, {"value": "0.0165", "module": "A5"}, {"value": "0.0769", "module": "C1"}, {"value": "0.206", "module": "C2"}, {"value": "0.605", "module": "C3"}, {"value": "0.286", "module": "C4"}, {"value": "-1.45", "module": "D", "scenario": "S0"}, {"value": "-1.4", "module": "D", "scenario": "S1"}]}, "resolvedFlowVersion": "38.00.000", "flowProperties": [], "typeOfFlow": "Other flow", "classification": {"classHierarchy": "Quantities / Environmental quantities / EPD EN 15804 / LCI indicators", "name": "GaBiCategories"}}, {"dataSetInternalID": 4, "referenceToFlowDataSet": {"shortDescription": [{"value": "Nicht-erneuerbare Primärenergie als Energieträger (PENRE)", "lang": "de"}, {"value": "Non renewable primary energy as energy carrier (PENRE)", "lang": "en"}], "type": "flow data set", "refObjectId": "ac857178-2b45-46ec-892a-a9a4332f0372", "uri": "../flows/ac857178-2b45-46ec-892a-a9a4332f0372.xml"}, "exchange direction": "INPUT", "other": {"anies": [{"name": "referenceToUnitGroupDataSet", "value": {"shortDescription": [{"value": "MJ", "lang": "de"}], "type": "unit group data set", "refObjectId": "93a60a57-a3c8-11da-a746-0800200c9a66", "uri": "../unitgroups/93a60a57-a3c8-11da-a746-0800200c9a66.xml"}}, {"value": "433.18", "module": "A1-A3"}, {"value": "20.1", "module": "A4"}, {"value": "1.91", "module": "A5"}, {"value": "1.3", "module": "C1"}, {"value": "3.46", "module": "C2"}, {"value": "7.55", "module": "C3"}, {"value": "1.9", "module": "C4"}, {"value": "-4.57", "module": "D", "scenario": "S0"}, {"value": "-2.69", "module": "D", "scenario": "S1"}]}, "resolvedFlowVersion": "38.00.000", "flowProperties": [], "typeOfFlow": "Other flow", "classification": {"classHierarchy": "Quantities", "name": "GaBiCategories"}}, {"dataSetInternalID": 5, "referenceToFlowDataSet": {"shortDescription": [{"value": "Nicht-erneuerbare Primärenergie zur stofflichen Nutzung (PENRM)", "lang": "de"}, {"value": "Non renewable primary energy as material utilization (PENRM)", "lang": "en"}], "type": "flow data set", "refObjectId": "1421caa0-679d-4bf4-b282-0eb850ccae27", "uri": "../flows/1421caa0-679d-4bf4-b282-0eb850ccae27.xml"}, "exchange direction": "INPUT", "other": {"anies": [{"name": "referenceToUnitGroupDataSet", "value": {"shortDescription": [{"value": "MJ", "lang": "de"}], "type": "unit group data set", "refObjectId": "93a60a57-a3c8-11da-a746-0800200c9a66", "uri": "../unitgroups/93a60a57-a3c8-11da-a746-0800200c9a66.xml"}}, {"value": "1.845", "module": "A1-A3"}, {"value": "0", "module": "A4"}, {"value": "-1.845", "module": "A5"}, {"value": "0", "module": "C1"}, {"value": "0", "module": "C2"}, {"value": "0", "module": "C3"}, {"value": "0", "module": "C4"}, {"value": "0", "module": "D", "scenario": "S0"}, {"value": "0", "module": "D", "scenario": "S1"}]}, "resolvedFlowVersion": "38.00.000", "flowProperties": [], "typeOfFlow": "Other flow", "classification": {"classHierarchy": "Quantities", "name": "GaBiCategories"}}, {"dataSetInternalID": 6, "referenceToFlowDataSet": {"shortDescription": [{"value": "Total nicht erneuerbare Primärenergie (PENRT)", "lang": "de"}, {"value": "Total use of non renewable primary energy resources (PENRT)", "lang": "en"}], "type": "flow data set", "refObjectId": "06159210-646b-4c8d-8583-da9b3b95a6c1", "uri": "../flows/06159210-646b-4c8d-8583-da9b3b95a6c1.xml"}, "exchange direction": "INPUT", "other": {"anies": [{"name": "referenceToUnitGroupDataSet", "value": {"shortDescription": [{"value": "MJ", "lang": "de"}], "type": "unit group data set", "refObjectId": "93a60a57-a3c8-11da-a746-0800200c9a66", "uri": "../unitgroups/93a60a57-a3c8-11da-a746-0800200c9a66.xml"}}, {"value": "435.02", "module": "A1-A3"}, {"value": "20.1", "module": "A4"}, {"value": "0.0716", "module": "A5"}, {"value": "1.3", "module": "C1"}, {"value": "3.46", "module": "C2"}, {"value": "7.55", "module": "C3"}, {"value": "1.9", "module": "C4"}, {"value": "-4.57", "module": "D", "scenario": "S0"}, {"value": "-2.69", "module": "D", "scenario": "S1"}]}, "resolvedFlowVersion": "38.00.000", "flowProperties": [], "typeOfFlow": "Other flow", "classification": {"classHierarchy": "Quantities / Environmental quantities / EPD EN 15804 / LCI indicators", "name": "GaBiCategories"}}, {"dataSetInternalID": 7, "referenceToFlowDataSet": {"shortDescription": [{"value": "Einsatz von Sekundärstoffen (SM)", "lang": "de"}, {"value": "Use of secondary material (SM)", "lang": "en"}], "type": "flow data set", "refObjectId": "c6a1f35f-2d09-4f54-8dfb-97e502e1ce92", "uri": "../flows/c6a1f35f-2d09-4f54-8dfb-97e502e1ce92.xml"}, "exchange direction": "INPUT", "other": {"anies": [{"name": "referenceToUnitGroupDataSet", "value": {"shortDescription": [{"value": "kg", "lang": "de"}], "type": "unit group data set", "refObjectId": "ad38d542-3fe9-439d-9b95-2f5f7752acaf", "uri": "../unitgroups/ad38d542-3fe9-439d-9b95-2f5f7752acaf.xml"}}, {"value": "4.72", "module": "A1-A3"}, {"value": "0", "module": "A4"}, {"value": "0", "module": "A5"}, {"value": "0", "module": "C1"}, {"value": "0", "module": "C2"}, {"value": "149.03", "module": "C3"}, {"value": "0", "module": "C4"}, {"value": "0", "module": "D", "scenario": "S0"}, {"value": "0", "module": "D", "scenario": "S1"}]}, "resolvedFlowVersion": "38.00.000", "flowProperties": [], "typeOfFlow": "Other flow", "classification": {"classHierarchy": "Quantities / Environmental quantities / EPD EN 15804 / LCI indicators", "name": "GaBiCategories"}}, {"dataSetInternalID": 8, "referenceToFlowDataSet": {"shortDescription": [{"value": "Erneuerbare Sekundärbrennstoffe (RSF)", "lang": "de"}, {"value": "Use of renewable secondary fuels (RSF)", "lang": "en"}], "type": "flow data set", "refObjectId": "64333088-a55f-4aa2-9a31-c10b07816787", "uri": "../flows/64333088-a55f-4aa2-9a31-c10b07816787.xml"}, "exchange direction": "INPUT", "other": {"anies": [{"name": "referenceToUnitGroupDataSet", "value": {"shortDescription": [{"value": "MJ", "lang": "de"}], "type": "unit group data set", "refObjectId": "93a60a57-a3c8-11da-a746-0800200c9a66", "uri": "../unitgroups/93a60a57-a3c8-11da-a746-0800200c9a66.xml"}}, {"value": "0", "module": "A1-A3"}, {"value": "0", "module": "A4"}, {"value": "0", "module": "A5"}, {"value": "0", "module": "C1"}, {"value": "0", "module": "C2"}, {"value": "0", "module": "C3"}, {"value": "0", "module": "C4"}, {"value": "0", "module": "D", "scenario": "S0"}, {"value": "0", "module": "D", "scenario": "S1"}]}, "resolvedFlowVersion": "38.00.000", "flowProperties": [], "typeOfFlow": "Other flow", "classification": {"classHierarchy": "Quantities / Environmental quantities / EPD EN 15804 / LCI indicators", "name": "GaBiCategories"}}, {"dataSetInternalID": 9, "referenceToFlowDataSet": {"shortDescription": [{"value": "Nicht erneuerbare Sekundärbrennstoffe (NRSF)", "lang": "de"}, {"value": "Use of non renewable secondary fuels (NRSF)", "lang": "en"}], "type": "flow data set", "refObjectId": "89def144-d39a-4287-b86f-efde453ddcb2", "uri": "../flows/89def144-d39a-4287-b86f-efde453ddcb2.xml"}, "exchange direction": "INPUT", "other": {"anies": [{"name": "referenceToUnitGroupDataSet", "value": {"shortDescription": [{"value": "MJ", "lang": "de"}], "type": "unit group data set", "refObjectId": "93a60a57-a3c8-11da-a746-0800200c9a66", "uri": "../unitgroups/93a60a57-a3c8-11da-a746-0800200c9a66.xml"}}, {"value": "0", "module": "A1-A3"}, {"value": "0", "module": "A4"}, {"value": "0", "module": "A5"}, {"value": "0", "module": "C1"}, {"value": "0", "module": "C2"}, {"value": "0", "module": "C3"}, {"value": "0", "module": "C4"}, {"value": "0", "module": "D", "scenario": "S0"}, {"value": "0", "module": "D", "scenario": "S1"}]}, "resolvedFlowVersion": "38.00.000", "flowProperties": [], "typeOfFlow": "Other flow", "classification": {"classHierarchy": "Quantities / Environmental quantities / EPD EN 15804 / LCI indicators", "name": "GaBiCategories"}}, {"dataSetInternalID": 10, "referenceToFlowDataSet": {"shortDescription": [{"value": "Einsatz von Süßwasserressourcen (FW)", "lang": "de"}, {"value": "Use of net fresh water (FW)", "lang": "en"}], "type": "flow data set", "refObjectId": "3cf952c8-f3a4-461d-8c96-96456ca62246", "uri": "../flows/3cf952c8-f3a4-461d-8c96-96456ca62246.xml"}, "exchange direction": "INPUT", "other": {"anies": [{"name": "referenceToUnitGroupDataSet", "value": {"shortDescription": [{"value": "m^3", "lang": "de"}], "type": "unit group data set", "refObjectId": "cd950537-0a98-4044-9ba7-9f9a68d0a504", "uri": "../unitgroups/cd950537-0a98-4044-9ba7-9f9a68d0a504.xml"}}, {"value": "0.02", "module": "A1-A3"}, {"value": "0.00104", "module": "A4"}, {"value": "0.000981", "module": "A5"}, {"value": "6.7E-05", "module": "C1"}, {"value": "0.000179", "module": "C2"}, {"value": "0.00211", "module": "C3"}, {"value": "0.00048", "module": "C4"}, {"value": "-0.000765", "module": "D", "scenario": "S0"}, {"value": "-0.00152", "module": "D", "scenario": "S1"}]}, "resolvedFlowVersion": "38.00.000", "flowProperties": [], "typeOfFlow": "Other flow", "classification": {"classHierarchy": "Quantities / Environmental quantities / EPD EN 15804 / LCI indicators", "name": "GaBiCategories"}}, {"dataSetInternalID": 11, "referenceToFlowDataSet": {"shortDescription": [{"value": "Gefährlicher Abfall zur Deponie (HWD)", "lang": "de"}, {"value": "Hazardous waste disposed (HWD)", "lang": "en"}], "type": "flow data set", "refObjectId": "430f9e0f-59b2-46a0-8e0d-55e0e84948fc", "uri": "../flows/430f9e0f-59b2-46a0-8e0d-55e0e84948fc.xml"}, "exchange direction": "OUTPUT", "other": {"anies": [{"name": "referenceToUnitGroupDataSet", "value": {"shortDescription": [{"value": "kg", "lang": "de"}], "type": "unit group data set", "refObjectId": "ad38d542-3fe9-439d-9b95-2f5f7752acaf", "uri": "../unitgroups/ad38d542-3fe9-439d-9b95-2f5f7752acaf.xml"}}, {"value": "1.152659E-07", "module": "A1-A3"}, {"value": "9.28E-11", "module": "A4"}, {"value": "6.96E-12", "module": "A5"}, {"value": "5.99E-12", "module": "C1"}, {"value": "1.6E-11", "module": "C2"}, {"value": "9.44E-11", "module": "C3"}, {"value": "9.76E-11", "module": "C4"}, {"value": "-2.02E-10", "module": "D", "scenario": "S0"}, {"value": "-5.1E-10", "module": "D", "scenario": "S1"}]}, "resolvedFlowVersion": "38.00.000", "flowProperties": [], "typeOfFlow": "Other flow", "classification": {"classHierarchy": "Quantities / Environmental quantities / EPD EN 15804 / LCI indicators", "name": "GaBiCategories"}}, {"dataSetInternalID": 12, "referenceToFlowDataSet": {"shortDescription": [{"value": "Entsorgter nicht gefährlicher Abfall (NHWD)", "lang": "de"}, {"value": "Non hazardous waste disposed (NHWD)", "lang": "en"}], "type": "flow data set", "refObjectId": "b29ef66b-e286-4afa-949f-62f1a7b4d7fa", "uri": "../flows/b29ef66b-e286-4afa-949f-62f1a7b4d7fa.xml"}, "exchange direction": "OUTPUT", "other": {"anies": [{"name": "referenceToUnitGroupDataSet", "value": {"shortDescription": [{"value": "kg", "lang": "de"}], "type": "unit group data set", "refObjectId": "ad38d542-3fe9-439d-9b95-2f5f7752acaf", "uri": "../unitgroups/ad38d542-3fe9-439d-9b95-2f5f7752acaf.xml"}}, {"value": "0.44447", "module": "A1-A3"}, {"value": "0.00318", "module": "A4"}, {"value": "0.00512", "module": "A5"}, {"value": "0.000205", "module": "C1"}, {"value": "0.000548", "module": "C2"}, {"value": "0.002", "module": "C3"}, {"value": "0.002", "module": "C4"}, {"value": "-3.1", "module": "D", "scenario": "S0"}, {"value": "-0.00191", "module": "D", "scenario": "S1"}]}, "resolvedFlowVersion": "38.00.000", "flowProperties": [], "typeOfFlow": "Other flow", "classification": {"classHierarchy": "Quantities / Environmental quantities / EPD EN 15804 / LCI indicators", "name": "GaBiCategories"}}, {"dataSetInternalID": 13, "referenceToFlowDataSet": {"shortDescription": [{"value": "Entsorgter radioaktiver Abfall (RWD)", "lang": "de"}, {"value": "Radioactive waste disposed (RWD)", "lang": "en"}], "type": "flow data set", "refObjectId": "3449546e-52ad-4b39-b809-9fb77cea8ff6", "uri": "../flows/3449546e-52ad-4b39-b809-9fb77cea8ff6.xml"}, "exchange direction": "OUTPUT", "other": {"anies": [{"name": "referenceToUnitGroupDataSet", "value": {"shortDescription": [{"value": "kg", "lang": "de"}], "type": "unit group data set", "refObjectId": "ad38d542-3fe9-439d-9b95-2f5f7752acaf", "uri": "../unitgroups/ad38d542-3fe9-439d-9b95-2f5f7752acaf.xml"}}, {"value": "0.00331733", "module": "A1-A3"}, {"value": "2.02E-05", "module": "A4"}, {"value": "4.09E-06", "module": "A5"}, {"value": "1.3E-06", "module": "C1"}, {"value": "3.48E-06", "module": "C2"}, {"value": "9.95E-05", "module": "C3"}, {"value": "9.95E-05", "module": "C4"}, {"value": "-0.000143", "module": "D", "scenario": "S0"}, {"value": "-0.000122", "module": "D", "scenario": "S1"}]}, "resolvedFlowVersion": "38.00.000", "flowProperties": [], "typeOfFlow": "Other flow", "classification": {"classHierarchy": "Quantities / Environmental quantities / EPD EN 15804 / LCI indicators", "name": "GaBiCategories"}}, {"dataSetInternalID": 14, "referenceToFlowDataSet": {"shortDescription": [{"value": "Komponenten für die Wiederverwendung (CRU)", "lang": "de"}, {"value": "Components for re-use (CRU)", "lang": "en"}], "type": "flow data set", "refObjectId": "a2b32f97-3fc7-4af2-b209-525bc6426f33", "uri": "../flows/a2b32f97-3fc7-4af2-b209-525bc6426f33.xml"}, "exchange direction": "OUTPUT", "other": {"anies": [{"name": "referenceToUnitGroupDataSet", "value": {"shortDescription": [{"value": "kg", "lang": "de"}], "type": "unit group data set", "refObjectId": "ad38d542-3fe9-439d-9b95-2f5f7752acaf", "uri": "../unitgroups/ad38d542-3fe9-439d-9b95-2f5f7752acaf.xml"}}, {"value": "0", "module": "A1-A3"}, {"value": "0", "module": "A4"}, {"value": "0", "module": "A5"}, {"value": "0", "module": "C1"}, {"value": "0", "module": "C2"}, {"value": "0", "module": "C3"}, {"value": "0", "module": "C4"}, {"value": "0", "module": "D", "scenario": "S0"}, {"value": "0", "module": "D", "scenario": "S1"}]}, "resolvedFlowVersion": "38.00.000", "flowProperties": [], "typeOfFlow": "Other flow", "classification": {"classHierarchy": "Quantities / Environmental quantities / EPD EN 15804 / LCI indicators", "name": "GaBiCategories"}}, {"dataSetInternalID": 15, "referenceToFlowDataSet": {"shortDescription": [{"value": "Stoffe zum Recycling (MFR)", "lang": "de"}, {"value": "Materials for recycling (MFR)", "lang": "en"}], "type": "flow data set", "refObjectId": "d7fe48a5-4103-49c8-9aae-b0b5dfdbd6ae", "uri": "../flows/d7fe48a5-4103-49c8-9aae-b0b5dfdbd6ae.xml"}, "exchange direction": "OUTPUT", "other": {"anies": [{"name": "referenceToUnitGroupDataSet", "value": {"shortDescription": [{"value": "kg", "lang": "de"}], "type": "unit group data set", "refObjectId": "ad38d542-3fe9-439d-9b95-2f5f7752acaf", "uri": "../unitgroups/ad38d542-3fe9-439d-9b95-2f5f7752acaf.xml"}}, {"value": "0", "module": "A1-A3"}, {"value": "0", "module": "A4"}, {"value": "0", "module": "A5"}, {"value": "0", "module": "C1"}, {"value": "0", "module": "C2"}, {"value": "0", "module": "C3"}, {"value": "0", "module": "C4"}, {"value": "0", "module": "D", "scenario": "S0"}, {"value": "0", "module": "D", "scenario": "S1"}]}, "resolvedFlowVersion": "38.00.000", "flowProperties": [], "typeOfFlow": "Other flow", "classification": {"classHierarchy": "Quantities / Environmental quantities / EPD EN 15804 / LCI indicators", "name": "GaBiCategories"}}, {"dataSetInternalID": 16, "referenceToFlowDataSet": {"shortDescription": [{"value": "Stoffe für die Energierückgewinnung (MER)", "lang": "de"}, {"value": "Materials for energy recovery (MER)", "lang": "en"}], "type": "flow data set", "refObjectId": "59a9181c-3aaf-46ee-8b13-2b3723b6e447", "uri": "../flows/59a9181c-3aaf-46ee-8b13-2b3723b6e447.xml"}, "exchange direction": "OUTPUT", "other": {"anies": [{"name": "referenceToUnitGroupDataSet", "value": {"shortDescription": [{"value": "kg", "lang": "de"}], "type": "unit group data set", "refObjectId": "ad38d542-3fe9-439d-9b95-2f5f7752acaf", "uri": "../unitgroups/ad38d542-3fe9-439d-9b95-2f5f7752acaf.xml"}}, {"value": "0", "module": "A1-A3"}, {"value": "0", "module": "A4"}, {"value": "0", "module": "A5"}, {"value": "0", "module": "C1"}, {"value": "0", "module": "C2"}, {"value": "0", "module": "C3"}, {"value": "0", "module": "C4"}, {"value": "0", "module": "D", "scenario": "S0"}, {"value": "0", "module": "D", "scenario": "S1"}]}, "resolvedFlowVersion": "38.00.000", "flowProperties": [], "typeOfFlow": "Other flow", "classification": {"classHierarchy": "Quantities / Environmental quantities / EPD EN 15804 / LCI indicators", "name": "GaBiCategories"}}, {"dataSetInternalID": 17, "referenceToFlowDataSet": {"shortDescription": [{"value": "Exportierte elektrische Energie (EEE)", "lang": "de"}, {"value": "Exported electrical energy (EEE)", "lang": "en"}], "type": "flow data set", "refObjectId": "4da0c987-2b76-40d6-9e9e-82a017aaaf29", "uri": "../flows/4da0c987-2b76-40d6-9e9e-82a017aaaf29.xml"}, "exchange direction": "OUTPUT", "other": {"anies": [{"name": "referenceToUnitGroupDataSet", "value": {"shortDescription": [{"value": "MJ", "lang": "de"}], "type": "unit group data set", "refObjectId": "93a60a57-a3c8-11da-a746-0800200c9a66", "uri": "../unitgroups/93a60a57-a3c8-11da-a746-0800200c9a66.xml"}}, {"value": "0", "module": "A1-A3"}, {"value": "0", "module": "A4"}, {"value": "0.794", "module": "A5"}, {"value": "0", "module": "C1"}, {"value": "0", "module": "C2"}, {"value": "0", "module": "C3"}, {"value": "0", "module": "C4"}, {"value": "0", "module": "D", "scenario": "S0"}, {"value": "0", "module": "D", "scenario": "S1"}]}, "resolvedFlowVersion": "38.00.000", "flowProperties": [], "typeOfFlow": "Other flow", "classification": {"classHierarchy": "Quantities / Environmental quantities / EPD EN 15804 / LCI indicators", "name": "GaBiCategories"}}, {"dataSetInternalID": 18, "referenceToFlowDataSet": {"shortDescription": [{"value": "Exportierte thermische Energie (EET)", "lang": "de"}, {"value": "Exported thermal energy (EET)", "lang": "en"}], "type": "flow data set", "refObjectId": "98daf38a-7a79-46d3-9a37-2b7bd0955810", "uri": "../flows/98daf38a-7a79-46d3-9a37-2b7bd0955810.xml"}, "exchange direction": "OUTPUT", "other": {"anies": [{"name": "referenceToUnitGroupDataSet", "value": {"shortDescription": [{"value": "MJ", "lang": "de"}], "type": "unit group data set", "refObjectId": "93a60a57-a3c8-11da-a746-0800200c9a66", "uri": "../unitgroups/93a60a57-a3c8-11da-a746-0800200c9a66.xml"}}, {"value": "0", "module": "A1-A3"}, {"value": "0", "module": "A4"}, {"value": "1.42", "module": "A5"}, {"value": "0", "module": "C1"}, {"value": "0", "module": "C2"}, {"value": "0", "module": "C3"}, {"value": "0", "module": "C4"}, {"value": "0", "module": "D", "scenario": "S0"}, {"value": "0", "module": "D", "scenario": "S1"}]}, "resolvedFlowVersion": "38.00.000", "flowProperties": [], "typeOfFlow": "Other flow", "classification": {"classHierarchy": "Quantities / Environmental quantities / EPD EN 15804 / LCI indicators", "name": "GaBiCategories"}}]}, "LCIAResults": {"LCIAResult": [{"referenceToLCIAMethodDataSet": {"shortDescription": [{"value": "Globales Erwärmungspotenzial total (GWP-total)", "lang": "de"}, {"value": "Global Warming Potential total (GWP-total)", "lang": "en"}], "type": "LCIA method data set", "refObjectId": "6a37f984-a4b3-458a-a20a-64418c145fa2", "uri": "../lciamethods/6a37f984-a4b3-458a-a20a-64418c145fa2.xml"}, "other": {"anies": [{"name": "referenceToUnitGroupDataSet", "value": {"shortDescription": [{"value": "kg CO_(2)-Äq.", "lang": "de"}], "type": "unit group data set", "refObjectId": "1ebf3012-d0db-4de2-aefd-ef30cedb0be1", "uri": "../unitgroups/1ebf3012-d0db-4de2-aefd-ef30cedb0be1.xml"}}, {"value": "27.651", "module": "A1-A3"}, {"value": "1.52", "module": "A4"}, {"value": "0.441", "module": "A5"}, {"value": "0.0975", "module": "C1"}, {"value": "0.261", "module": "C2"}, {"value": "0.387", "module": "C3"}, {"value": "0.141", "module": "C4"}, {"value": "-0.347", "module": "D", "scenario": "S0"}, {"value": "-0.182", "module": "D", "scenario": "S1"}]}}, {"referenceToLCIAMethodDataSet": {"shortDescription": [{"value": "Globales Erwärmungspotenzial fossil (GWP-fossil)", "lang": "de"}, {"value": "Global Warming Potential fossil fuels (GWP-fossil)", "lang": "en"}], "type": "LCIA method data set", "refObjectId": "5f635281-343e-44fb-83df-1971b155e6b6", "uri": "../lciamethods/5f635281-343e-44fb-83df-1971b155e6b6.xml"}, "other": {"anies": [{"name": "referenceToUnitGroupDataSet", "value": {"shortDescription": [{"value": "kg CO_(2)-Äq.", "lang": "de"}], "type": "unit group data set", "refObjectId": "1ebf3012-d0db-4de2-aefd-ef30cedb0be1", "uri": "../unitgroups/1ebf3012-d0db-4de2-aefd-ef30cedb0be1.xml"}}, {"value": "27.538", "module": "A1-A3"}, {"value": "1.51", "module": "A4"}, {"value": "0.285", "module": "A5"}, {"value": "0.101", "module": "C1"}, {"value": "0.26", "module": "C2"}, {"value": "0.385", "module": "C3"}, {"value": "0.145", "module": "C4"}, {"value": "-0.346", "module": "D", "scenario": "S0"}, {"value": "-0.18", "module": "D", "scenario": "S1"}]}}, {"referenceToLCIAMethodDataSet": {"shortDescription": [{"value": "Globales Erwärmungspotenzial biogen (GWP-biogenic)", "lang": "de"}, {"value": "Global Warming Potential biogenic (GWP-biogenic)", "lang": "en"}], "type": "LCIA method data set", "refObjectId": "2356e1ab-0185-4db5-86e5-16de51c7485c", "uri": "../lciamethods/2356e1ab-0185-4db5-86e5-16de51c7485c.xml"}, "other": {"anies": [{"name": "referenceToUnitGroupDataSet", "value": {"shortDescription": [{"value": "kg CO_(2)-Äq.", "lang": "de"}], "type": "unit group data set", "refObjectId": "1ebf3012-d0db-4de2-aefd-ef30cedb0be1", "uri": "../unitgroups/1ebf3012-d0db-4de2-aefd-ef30cedb0be1.xml"}}, {"value": "0.0447", "module": "A1-A3"}, {"value": "0.000621", "module": "A4"}, {"value": "0.156", "module": "A5"}, {"value": "-0.0043", "module": "C1"}, {"value": "0.000107", "module": "C2"}, {"value": "6.6E-05", "module": "C3"}, {"value": "0.00429", "module": "C4"}, {"value": "-0.000211", "module": "D", "scenario": "S0"}, {"value": "-0.00185", "module": "D", "scenario": "S1"}]}}, {"referenceToLCIAMethodDataSet": {"shortDescription": [{"value": "Globales Erwärmungspotenzial luluc (GWP-luluc)", "lang": "de"}, {"value": "Global Warming Potential luluc (GWP-luluc)", "lang": "en"}], "type": "LCIA method data set", "refObjectId": "4331bbdb-978a-490d-8707-eeb047f01a55", "uri": "../lciamethods/4331bbdb-978a-490d-8707-eeb047f01a55.xml"}, "other": {"anies": [{"name": "referenceToUnitGroupDataSet", "value": {"shortDescription": [{"value": "kg CO_(2)-Äq.", "lang": "de"}], "type": "unit group data set", "refObjectId": "1ebf3012-d0db-4de2-aefd-ef30cedb0be1", "uri": "../unitgroups/1ebf3012-d0db-4de2-aefd-ef30cedb0be1.xml"}}, {"value": "0.004991", "module": "A1-A3"}, {"value": "0.00563", "module": "A4"}, {"value": "8.64E-07", "module": "A5"}, {"value": "0.000363", "module": "C1"}, {"value": "0.00097", "module": "C2"}, {"value": "0.00178", "module": "C3"}, {"value": "0.000267", "module": "C4"}, {"value": "-0.000793", "module": "D", "scenario": "S0"}, {"value": "-4.35E-05", "module": "D", "scenario": "S1"}]}}, {"referenceToLCIAMethodDataSet": {"shortDescription": [{"value": "Abbau Potential der stratosphärischen Ozonschicht (ODP)", "lang": "de"}, {"value": "Depletion potential of the stratospheric ozone layer (ODP)", "lang": "en"}], "type": "LCIA method data set", "refObjectId": "b5c629d6-def3-11e6-bf01-fe55135034f3", "uri": "../lciamethods/b5c629d6-def3-11e6-bf01-fe55135034f3.xml"}, "other": {"anies": [{"name": "referenceToUnitGroupDataSet", "value": {"shortDescription": [{"value": "kg CFC11-Äq.", "lang": "de"}], "type": "unit group data set", "refObjectId": "d9e957c9-7309-4474-bf3a-7777df6c4e5b", "uri": "../unitgroups/d9e957c9-7309-4474-bf3a-7777df6c4e5b.xml"}}, {"value": "2.2626195E-09", "module": "A1-A3"}, {"value": "2.15E-13", "module": "A4"}, {"value": "2.62E-14", "module": "A5"}, {"value": "1.39E-14", "module": "C1"}, {"value": "3.71E-14", "module": "C2"}, {"value": "5.74E-13", "module": "C3"}, {"value": "3.44E-13", "module": "C4"}, {"value": "-2.75E-12", "module": "D", "scenario": "S0"}, {"value": "-3.07E-12", "module": "D", "scenario": "S1"}]}}, {"referenceToLCIAMethodDataSet": {"shortDescription": [{"value": "Versauerungspotenzial von Boden und Wasser (AP)", "lang": "de"}, {"value": "Acidification potential of land and water (AP)", "lang": "en"}], "type": "LCIA method data set", "refObjectId": "b5c611c6-def3-11e6-bf01-fe55135034f3", "uri": "../lciamethods/b5c611c6-def3-11e6-bf01-fe55135034f3.xml"}, "other": {"anies": [{"name": "referenceToUnitGroupDataSet", "value": {"shortDescription": [{"value": "mol H^(+)-Äq.", "lang": "de"}], "type": "unit group data set", "refObjectId": "42e089ac-92bf-4bf2-8ca1-5fc40d18f2ed", "uri": "../unitgroups/42e089ac-92bf-4bf2-8ca1-5fc40d18f2ed.xml"}}, {"value": "0.02262", "module": "A1-A3"}, {"value": "0.00134", "module": "A4"}, {"value": "6.32E-05", "module": "A5"}, {"value": "0.000475", "module": "C1"}, {"value": "0.000231", "module": "C2"}, {"value": "0.00199", "module": "C3"}, {"value": "0.00103", "module": "C4"}, {"value": "-0.00115", "module": "D", "scenario": "S0"}, {"value": "-0.000191", "module": "D", "scenario": "S1"}]}}, {"referenceToLCIAMethodDataSet": {"shortDescription": [{"value": "Eutrophierungspotenzial Süßwasser (EP-freshwater)", "lang": "de"}, {"value": "Eutrophication potential aquatic freshwater (EP-freshwater)", "lang": "en"}], "type": "LCIA method data set", "refObjectId": "b53ec18f-7377-4ad3-86eb-cc3f4f276b2b", "uri": "../lciamethods/b53ec18f-7377-4ad3-86eb-cc3f4f276b2b.xml"}, "other": {"anies": [{"name": "referenceToUnitGroupDataSet", "value": {"shortDescription": [{"value": "kg P-Äq.", "lang": "de"}], "type": "unit group data set", "refObjectId": "0429039d-a61d-4590-ba67-aa4a20a810a1", "uri": "../unitgroups/0429039d-a61d-4590-ba67-aa4a20a810a1.xml"}}, {"value": "2.606E-05", "module": "A1-A3"}, {"value": "3.12E-06", "module": "A4"}, {"value": "7.24E-09", "module": "A5"}, {"value": "2.01E-07", "module": "C1"}, {"value": "5.38E-07", "module": "C2"}, {"value": "1.11E-06", "module": "C3"}, {"value": "2.46E-07", "module": "C4"}, {"value": "-9.8E-07", "module": "D", "scenario": "S0"}, {"value": "-5.65E-07", "module": "D", "scenario": "S1"}]}}, {"referenceToLCIAMethodDataSet": {"shortDescription": [{"value": "Eutrophierungspotenzial Salzwasser (EP-marine)", "lang": "de"}, {"value": "Eutrophication potential aquatic marine (EP-marine)", "lang": "en"}], "type": "LCIA method data set", "refObjectId": "b5c619fa-def3-11e6-bf01-fe55135034f3", "uri": "../lciamethods/b5c619fa-def3-11e6-bf01-fe55135034f3.xml"}, "other": {"anies": [{"name": "referenceToUnitGroupDataSet", "value": {"shortDescription": [{"value": "kg N-Äq.", "lang": "de"}], "type": "unit group data set", "refObjectId": "d05bb823-ecdf-4686-8c40-bf1d9257859f", "uri": "../unitgroups/d05bb823-ecdf-4686-8c40-bf1d9257859f.xml"}}, {"value": "0.008651", "module": "A1-A3"}, {"value": "0.000435", "module": "A4"}, {"value": "1.86E-05", "module": "A5"}, {"value": "0.000226", "module": "C1"}, {"value": "7.51E-05", "module": "C2"}, {"value": "0.00091", "module": "C3"}, {"value": "0.000262", "module": "C4"}, {"value": "-0.00045", "module": "D", "scenario": "S0"}, {"value": "-6.96E-05", "module": "D", "scenario": "S1"}]}}, {"referenceToLCIAMethodDataSet": {"shortDescription": [{"value": "Eutrophierungspotenzial Land (EP-terrestrial)", "lang": "de"}, {"value": "Eutrophication potential terrestrial (EP-terrestrial)", "lang": "en"}], "type": "LCIA method data set", "refObjectId": "b5c614d2-def3-11e6-bf01-fe55135034f3", "uri": "../lciamethods/b5c614d2-def3-11e6-bf01-fe55135034f3.xml"}, "other": {"anies": [{"name": "referenceToUnitGroupDataSet", "value": {"shortDescription": [{"value": "mol N-Äq.", "lang": "de"}], "type": "unit group data set", "refObjectId": "71b4d617-0ec9-4d3f-b65e-e438940c2401", "uri": "../unitgroups/71b4d617-0ec9-4d3f-b65e-e438940c2401.xml"}}, {"value": "0.09482", "module": "A1-A3"}, {"value": "0.00523", "module": "A4"}, {"value": "0.000291", "module": "A5"}, {"value": "0.0025", "module": "C1"}, {"value": "0.000902", "module": "C2"}, {"value": "0.01", "module": "C3"}, {"value": "0.00288", "module": "C4"}, {"value": "-0.00496", "module": "D", "scenario": "S0"}, {"value": "-0.000736", "module": "D", "scenario": "S1"}]}}, {"referenceToLCIAMethodDataSet": {"shortDescription": [{"value": "Bildungspotential für troposphärisches Ozon (POCP)", "lang": "de"}, {"value": "Formation potential of tropospheric ozone photochemical oxidants (POCP)", "lang": "en"}], "type": "LCIA method data set", "refObjectId": "b5c610fe-def3-11e6-bf01-fe55135034f3", "uri": "../lciamethods/b5c610fe-def3-11e6-bf01-fe55135034f3.xml"}, "other": {"anies": [{"name": "referenceToUnitGroupDataSet", "value": {"shortDescription": [{"value": "kg NMVOC-Äq.", "lang": "de"}], "type": "unit group data set", "refObjectId": "d27c25f8-fbc1-44c6-b47b-4adbae4199c6", "uri": "../unitgroups/d27c25f8-fbc1-44c6-b47b-4adbae4199c6.xml"}}, {"value": "0.024899", "module": "A1-A3"}, {"value": "0.00117", "module": "A4"}, {"value": "5.13E-05", "module": "A5"}, {"value": "0.000633", "module": "C1"}, {"value": "0.000201", "module": "C2"}, {"value": "0.00248", "module": "C3"}, {"value": "0.000798", "module": "C4"}, {"value": "-0.00106", "module": "D", "scenario": "S0"}, {"value": "-0.000177", "module": "D", "scenario": "S1"}]}}, {"referenceToLCIAMethodDataSet": {"shortDescription": [{"value": "Potenzial für den abiotischen Abbau nicht fossiler Ressourcen (ADPE)", "lang": "de"}, {"value": "Abiotic depletion potential for non fossil resources (ADPE)", "lang": "en"}], "type": "LCIA method data set", "refObjectId": "b2ad6494-c78d-11e6-9d9d-cec0c932ce01", "uri": "../lciamethods/b2ad6494-c78d-11e6-9d9d-cec0c932ce01.xml"}, "other": {"anies": [{"name": "referenceToUnitGroupDataSet", "value": {"shortDescription": [{"value": "kg Sb-Äq.", "lang": "de"}], "type": "unit group data set", "refObjectId": "54ccd2d9-a32a-4fc2-923d-f2c8c93e89d4", "uri": "../unitgroups/54ccd2d9-a32a-4fc2-923d-f2c8c93e89d4.xml"}}, {"value": "2.9271E-06", "module": "A1-A3"}, {"value": "1.56E-07", "module": "A4"}, {"value": "6.4E-10", "module": "A5"}, {"value": "1.01E-08", "module": "C1"}, {"value": "2.69E-08", "module": "C2"}, {"value": "4.27E-07", "module": "C3"}, {"value": "1.49E-08", "module": "C4"}, {"value": "-7.84E-08", "module": "D", "scenario": "S0"}, {"value": "-6.91E-08", "module": "D", "scenario": "S1"}]}}, {"referenceToLCIAMethodDataSet": {"shortDescription": [{"value": "Potenzial für den abiotischen Abbau fossiler Brennstoffe (ADPF)", "lang": "de"}, {"value": "Abiotic depletion potential for fossil resources (ADPF)", "lang": "en"}], "type": "LCIA method data set", "refObjectId": "b2ad6110-c78d-11e6-9d9d-cec0c932ce01", "uri": "../lciamethods/b2ad6110-c78d-11e6-9d9d-cec0c932ce01.xml"}, "other": {"anies": [{"name": "referenceToUnitGroupDataSet", "value": {"shortDescription": [{"value": "MJ", "lang": "de"}], "type": "unit group data set", "refObjectId": "93a60a57-a3c8-11da-a746-0800200c9a66", "uri": "../unitgroups/93a60a57-a3c8-11da-a746-0800200c9a66.xml"}}, {"value": "433.07", "module": "A1-A3"}, {"value": "20.1", "module": "A4"}, {"value": "0.0716", "module": "A5"}, {"value": "1.29", "module": "C1"}, {"value": "3.46", "module": "C2"}, {"value": "7.54", "module": "C3"}, {"value": "1.9", "module": "C4"}, {"value": "-4.56", "module": "D", "scenario": "S0"}, {"value": "-2.69", "module": "D", "scenario": "S1"}]}}, {"referenceToLCIAMethodDataSet": {"shortDescription": [{"value": "Wassernutzung (WDP)", "lang": "de"}, {"value": "Water use (WDP)", "lang": "en"}], "type": "LCIA method data set", "refObjectId": "b2ad66ce-c78d-11e6-9d9d-cec0c932ce01", "uri": "../lciamethods/b2ad66ce-c78d-11e6-9d9d-cec0c932ce01.xml"}, "other": {"anies": [{"name": "referenceToUnitGroupDataSet", "value": {"shortDescription": [{"value": "m^(3) Welt-Äq. entzogen", "lang": "de"}], "type": "unit group data set", "refObjectId": "6ae2df01-888e-46c8-b17d-49fa3869b476", "uri": "../unitgroups/6ae2df01-888e-46c8-b17d-49fa3869b476.xml"}}, {"value": "0.37273", "module": "A1-A3"}, {"value": "0.00592", "module": "A4"}, {"value": "0.0418", "module": "A5"}, {"value": "0.000382", "module": "C1"}, {"value": "0.00102", "module": "C2"}, {"value": "0.0744", "module": "C3"}, {"value": "0.0158", "module": "C4"}, {"value": "-0.00866", "module": "D", "scenario": "S0"}, {"value": "-0.00271", "module": "D", "scenario": "S1"}]}}, {"referenceToLCIAMethodDataSet": {"shortDescription": [{"value": "Auftreten von Krankheiten aufgrund von Feinstaubemissionen (PM)", "lang": "de"}, {"value": "Incidence of disease due to PM emissions (PM)", "lang": "en"}], "type": "LCIA method data set", "refObjectId": "b5c602c6-def3-11e6-bf01-fe55135034f3", "uri": "../lciamethods/b5c602c6-def3-11e6-bf01-fe55135034f3.xml"}, "other": {"anies": [{"name": "referenceToUnitGroupDataSet", "value": {"shortDescription": [{"value": "Krankheitsfälle", "lang": "de"}], "type": "unit group data set", "refObjectId": "3883559b-648f-4afc-8ba2-0bd24f3affa3", "uri": "../unitgroups/3883559b-648f-4afc-8ba2-0bd24f3affa3.xml"}}, {"module": "A1-A3"}, {"module": "A4"}, {"module": "A5"}, {"module": "C1"}, {"module": "C2"}, {"module": "C3"}, {"module": "C4"}, {"module": "D", "scenario": "S0"}, {"module": "D", "scenario": "S1"}]}}, {"referenceToLCIAMethodDataSet": {"shortDescription": [{"value": "Wirkung durch Exposition des Menschen mit U235 (IR)", "lang": "de"}, {"value": "Human exposure efficiency relative to U235 (IR)", "lang": "en"}], "type": "LCIA method data set", "refObjectId": "b5c632be-def3-11e6-bf01-fe55135034f3", "uri": "../lciamethods/b5c632be-def3-11e6-bf01-fe55135034f3.xml"}, "other": {"anies": [{"name": "referenceToUnitGroupDataSet", "value": {"shortDescription": [{"value": "kBq U235-Äq.", "lang": "de"}], "type": "unit group data set", "refObjectId": "456b05bf-1415-44a9-9993-02452f554c09", "uri": "../unitgroups/456b05bf-1415-44a9-9993-02452f554c09.xml"}}, {"module": "A1-A3"}, {"module": "A4"}, {"module": "A5"}, {"module": "C1"}, {"module": "C2"}, {"module": "C3"}, {"module": "C4"}, {"module": "D", "scenario": "S0"}, {"module": "D", "scenario": "S1"}]}}, {"referenceToLCIAMethodDataSet": {"shortDescription": [{"value": "Toxizitätsvergleichseinheit für Ökosysteme (ETP-fw)", "lang": "de"}, {"value": "Comparative toxic unit for ecosystems (ETP-fw)", "lang": "en"}], "type": "LCIA method data set", "refObjectId": "ee1082d1-b0f7-43ca-a1f0-21e2a4a74511", "uri": "../lciamethods/ee1082d1-b0f7-43ca-a1f0-21e2a4a74511.xml"}, "other": {"anies": [{"name": "referenceToUnitGroupDataSet", "value": {"shortDescription": [{"value": "CTUe", "lang": "de"}], "type": "unit group data set", "refObjectId": "aa959ded-f1eb-4efb-9c5c-2d60be36b3e6", "uri": "../unitgroups/aa959ded-f1eb-4efb-9c5c-2d60be36b3e6.xml"}}, {"module": "A1-A3"}, {"module": "A4"}, {"module": "A5"}, {"module": "C1"}, {"module": "C2"}, {"module": "C3"}, {"module": "C4"}, {"module": "D", "scenario": "S0"}, {"module": "D", "scenario": "S1"}]}}, {"referenceToLCIAMethodDataSet": {"shortDescription": [{"value": "Toxizitätsvergleichseinheit für Menschen (krebserregend) (HTP-c)", "lang": "de"}, {"value": "Comparative toxic unit for humans (carcinogenic) (HTP-c)", "lang": "en"}], "type": "LCIA method data set", "refObjectId": "2299222a-bbd8-474f-9d4f-4dd1f18aea7c", "uri": "../lciamethods/2299222a-bbd8-474f-9d4f-4dd1f18aea7c.xml"}, "other": {"anies": [{"name": "referenceToUnitGroupDataSet", "value": {"shortDescription": [{"value": "CTUh", "lang": "de"}], "type": "unit group data set", "refObjectId": "d4c9523e-2d7e-49fd-8469-998f547d3a70", "uri": "../unitgroups/d4c9523e-2d7e-49fd-8469-998f547d3a70.xml"}}, {"module": "A1-A3"}, {"module": "A4"}, {"module": "A5"}, {"module": "C1"}, {"module": "C2"}, {"module": "C3"}, {"module": "C4"}, {"module": "D", "scenario": "S0"}, {"module": "D", "scenario": "S1"}]}}, {"referenceToLCIAMethodDataSet": {"shortDescription": [{"value": "Toxizitätsvergleichseinheit für Menschen (nicht krebserregend) (HTP-nc)", "lang": "de"}, {"value": "Comparative toxic unit for humans (noncarcinogenic) (HTP-nc)", "lang": "en"}], "type": "LCIA method data set", "refObjectId": "3af763a5-b7a1-48c9-9cee-1f223481fcef", "uri": "../lciamethods/3af763a5-b7a1-48c9-9cee-1f223481fcef.xml"}, "other": {"anies": [{"name": "referenceToUnitGroupDataSet", "value": {"shortDescription": [{"value": "CTUh", "lang": "de"}], "type": "unit group data set", "refObjectId": "d4c9523e-2d7e-49fd-8469-998f547d3a70", "uri": "../unitgroups/d4c9523e-2d7e-49fd-8469-998f547d3a70.xml"}}, {"module": "A1-A3"}, {"module": "A4"}, {"module": "A5"}, {"module": "C1"}, {"module": "C2"}, {"module": "C3"}, {"module": "C4"}, {"module": "D", "scenario": "S0"}, {"module": "D", "scenario": "S1"}]}}, {"referenceToLCIAMethodDataSet": {"shortDescription": [{"value": "Bodenqualitätsindex (SQP)", "lang": "de"}, {"value": "Soil quality index (SQP)", "lang": "en"}], "type": "LCIA method data set", "refObjectId": "b2ad6890-c78d-11e6-9d9d-cec0c932ce01", "uri": "../lciamethods/b2ad6890-c78d-11e6-9d9d-cec0c932ce01.xml"}, "other": {"anies": [{"name": "referenceToUnitGroupDataSet", "value": {"shortDescription": [{"value": "SQP", "lang": "de"}], "type": "unit group data set", "refObjectId": "f130951c-e67f-4f7f-8dd4-665de3974e18", "uri": "../unitgroups/f130951c-e67f-4f7f-8dd4-665de3974e18.xml"}}, {"module": "A1-A3"}, {"module": "A4"}, {"module": "A5"}, {"module": "C1"}, {"module": "C2"}, {"module": "C3"}, {"module": "C4"}, {"module": "D", "scenario": "S0"}, {"module": "D", "scenario": "S1"}]}}]}, "otherAttributes": {"{http://www.indata.network/EPD/2019}epd-version": "1.2"}, "version": "1.1", "locations": "../ILCDLocations.xml"}