{"processInformation": {"dataSetInformation": {"UUID": "1a8ebb43-2e63-4fb6-a659-37f84dc5613e", "name": {"baseName": [{"value": "Nonwoven glass fibre wall covering", "lang": "en"}, {"value": "Glasvliestapete für Wand und Decke", "lang": "de"}], "functionalUnitFlowProperties": [{"lang": "en"}]}, "classificationInformation": {"classification": [{"class": [{"value": "Beschichtungen", "level": 0, "classId": "5"}, {"value": "Innenbeschichtungen", "level": 1, "classId": "5.5"}, {"value": "Wand- und Deckenbeläge", "level": 2, "classId": "5.5.01"}], "name": "OEKOBAU.DAT"}, {"class": [{"value": "02 Building products", "level": 0}, {"value": "Internal and external wall and ceiling finishes", "level": 1}, {"value": "Wall coverings", "level": 2}], "name": "IBUCategories"}]}, "generalComment": [{"value": "Nonwoven glass fibre wall covering, manufactured by Vitrulan Textile Glass GmbH, is made of glass yarns and used for both, functional and decorative purposes. It is generally distinguished from wall paperings based on a paper substrate by a high-quality special glass nonwoven which is used as the substrate material. The glass fibre wall covering has a virtually seamless, uniform appearance. Generally, it is glued on walls and ceilings and painted afterwards. It also includes white pigments to reduce processing time on the construction site. It is particularly easy to handle: it does not shrink or stretch, is easy to cut and produces perfect seams. It reinforces walls, covers smaller cracks, and prevents new smaller cracks from forming.\n\nDuring application, the wall or ceiling is pasted and then the strip of wall covering is hung on the prepared paste bed, or, alternatively, the wall covering comes with a water-activatable adhesive which is already applied to the wall coverings backing – this adhesive then can be easily activated by water using the Aqua-Quick device specially developed for this purpose. Vitrulans Aqua Technology facilitates work and reduces processing times for the user.\n\nSince nonwoven glass fibre wall coverings are designed to reinforce walls and ceilings, they are bonded to the buildings structure. This means that they are disposed of as construction waste. Waste arising from installation can generally be disposed of as household waste since glass fibre wall coverings are not classed as special waste. Our nonwoven wall covering is OEKO-TEX-certified and completely non-hazardous to health. Sustainable interior design and premium product quality are hallmarks of all our textile glass wall coverings.", "lang": "en"}, {"value": "Die Glasvliestapeten der Vitrulan Textile Glass GmbH werden aus Glasfilamenten hergestellt und sowohl für funktionale als auch für dekorative Zwecke verwendet. Sie unterscheiden sich generell von Tapeten auf Papierbasis durch ein hochwertiges Rohglasvlies, das als Trägermaterial verwendet wird. \n\nDie Glasvliestapete hat ein nahezu nahtloses, einheitliches Aussehen. Im Allgemeinen wird sie an Wände und Decken geklebt und anschließend gestrichen. Sie enthält auch Weißpigmente, um die Verarbeitungszeit auf der Baustelle zu verkürzen. Das Glasvlies ist besonders einfach zu verarbeiten: Es schrumpft nicht und dehnt sich nicht, lässt sich leicht schneiden und liefert perfekte Nähte. \n\nBei der Verarbeitung wird die Wand oder Decke mit Kleber versehen und dann eine Bahn der Glasvliestapete in das vorbereitete Kleberbett gelegt. Alternativ wird der Wandbelag mit einem wasseraktivierbaren Kleber geliefert, der bereits auf der Rückseite des Wandbelags aufgebracht ist - dieser Kleber kann dann mit dem speziell für diesen Zweck entwickelten 'Aqua-Quick-Gerät' einfach mit Wasser aktiviert werden. Die Aqua-Technologie von Vitrulan erleichtert die Arbeit und verkürzt die Verarbeitungszeiten für den Anwender. \n\nDa Glasvliestapeten zur Verstärkung von Wänden und Decken bestimmt sind, werden sie mit der Gebäudestruktur fest vereint. Das bedeutet, dass sie als Bauabfall entsorgt werden. Die bei der Installation anfallenden Abfälle können im Allgemeinen als Hausmüll entsorgt werden, da Glasfasertapeten nicht als Sondermüll eingestuft werden. Unsere Glasfasertapeten sind OEKO-TEX-zertifiziert und gesundheitlich völlig unbedenklich. Nachhaltige Innenraumgestaltung und erstklassige Produktqualität sind das Markenzeichen all unserer textilen Glasfaserwandbeläge.", "lang": "de"}]}, "quantitativeReference": {"referenceToReferenceFlow": [0]}, "time": {"referenceYear": 2024, "dataSetValidUntil": 2029, "other": {"anies": [{"name": "publicationDateOfEPD", "value": 1704758400000}]}}, "geography": {"locationOfOperationSupplyOrProduction": {"location": "RER"}}, "technology": {"technologyDescriptionAndIncludedProcesses": [{"value": "Nonwoven glass fibre wall covering, manufactured by Vitrulan Textile Glass GmbH, contains ca. 0.049 kg/m2 raw glass fleece and ca. 0.075 kg/m2 coating based on starch, polymeric materials and inorganic additives. It is produced in two main phases. Raw glass fleece manufacture: The basic components of a glass batch are silica sand, limestone, kaolin, and boric acid. These components are fused at approx. 1250˚C. The molten glass flows by gravity through the nozzles of a bushing plate made of platinum alloy to form filaments. A surface coating called a 'size' is applied to the individual filaments. The size largely determines the processing characteristics of the glass fibre material. The glass filaments are used to produce a raw glass fleece by means of a wetlaid production with chemical bonding. Product manufacture: The raw glass fleece is attributed a finishing treatment that completely coats the fleece. The finish is normally applied using a special technique in which both sides of the unprocessed fleece are impregnated and then dried. The finish determines essential product characteristics such as stability, cutting capability, flexibility, feel, and surface roughness. Basically, the finish primes the surface optimally for subsequent application and painting. The finish for our pre-pigmented glass fleeces contains high quality white pigments – this makes painting works on the construction site highly economically and significantly reduces labor and material costs. In the packing area, the dried and coated fleece is wound and shortened in line with customer specifications. In the packaging area, the picked wallpaper rolls are packaged individually before being sent for dispatch. \nTechnical data: \nMain characteristics of our nonwoven glass fibre wall covering are:\nSuperb reaction to fire: B-s1, d0 according to DIN EN 13501-1\nWall reinforcing and crack bridging: class A1 according to Bundesausschuss Farbe und Sachwertschutz data sheet (BFS-Merkblatt) No. 19\nImpact and perforation resistant\nAbrasion and scrub resistant (depending on the coating)\nResistant to disinfectants and cleaning agents (depending on the coating)\nNon-toxic and food-safe: OEKO-TEX-certified\nWater vapour permeable\nSuitable for allergy sufferers\nIn addition to the many technical benefits, nonwoven glass fibre wall covering provides almost limitless scope for creativity when it comes to interior design \nDeclared unit: \nThe declared unit refers to 1 m2 of nonwoven glass fibre wall covering with an area weight of 0.124 kg/m.", "lang": "en"}, {"value": "Die von der Vitrulan Textile Glass GmbH hergestellte Glasvliestapete für Wand und Decke enthält ca. 0,049 kg/m2 Rohglasvlies und ca. 0,075 kg/m2 Beschichtung auf Stärkebasis mit polymeren Materialien und anorganischen Zusätzen. Der Wandbelag wird in zwei Hauptphasen hergestellt.\n\nHerstellung des Rohglasvlieses: Die Grundbestandteile der Glasmasse sind Quarzsand, Kalkstein, Kaolin und Borsäure. Die Komponenten werden bei ca. 1250˚C geschmolzen. Durch die Schwerkraft fließt die heiße Glasmasse durch die Düsenbohrungen einer Platinspinnplatte. Bevor die einzelnen Filamente zu einem Spinnfaden gebündelt werden, wird eine sog. Schlichte aufgetragen. Dies ist eine oberflächliche Beschichtung, die auf die Fasern aufgebracht wird und bestimmt im hohen Maße die Verarbeitungseigenschaften des Glasfasermaterials. Aus den Glasfilamenten wird in einem Nassvliesverfahren mit chemischer Bindung ein Rohglasvlies hergestellt.\n\nHerstellung des Produkts: Das Rohglasvlies wird mit einer Veredelung versehen, die das Vlies vollständig umhüllt. Die Veredelung erfolgt in der Regel durch ein spezielles Verfahren, bei dem beide Seiten des unbearbeiteten Rohglasvlieses imprägniert und anschließend getrocknet werden. Die Ausrüstung bestimmt wesentliche Produkteigenschaften wie Stabilität, Schnittfähigkeit, Flexibilität, Griff und Oberflächenrauhigkeit. Grundsätzlich bereitet die Ausrüstung die Oberfläche optimal für die anschließende Applikation und Farbbeschichtung vor. Im Verpackungsbereich wird das getrocknete und beschichtete Vlies nach Kundenwunsch gewickelt und gekürzt. Im Verpackungsbereich werden die kommissionierten Tapetenrollen einzeln verpackt, bevor sie in den Versand gehen. \nTechnische Daten: \nDie wichtigsten Eigenschaften unser Glasvliestapete für Wand und Decke sind: \n- Hervorragendes Brandverhalten: B-s1, d0 nach DIN EN 13501-1\n- Wandarmierung und Rissüberbrückung: Klasse A1 nach BFS-Merkblatt Nr. 19 \n- Stoß- und durchstoßfest\n- Abrieb- und scheuerfest (in Abhängigkeit von der Beschichtung) \n- Desinfektions- und Reinigungsmittelbeständig (in Abhängigkeit von der Beschichtung)\n- Schadstofffrei und lebensmittelecht: OEKO-TEX-zertifiziert\n- Wasserdampfdurchlässig\n- Für Allergiker geeignet\n\nNeben den vielen technischen Vorteilen bietet die Glasvliestapete einen nahezu grenzenlosen Spielraum für Kreativität bei der Raumgestaltung. \nDeklarierte Einheit: \nDie angegebene Einheit bezieht sich auf 1 m2 Glasvliestapete für Wand und Decke mit einem Flächengewicht von 0,124 kg/m².", "lang": "de"}], "technologicalApplicability": [{"value": "Nonwoven glass fibre wall coverings are used indoors on ceilings and walls in the following steps. More details are to be found in the technical data sheets.\n\nPREPARATION: Substrates should be dry, clean, smooth and stable. Pretreat absorbent substrates with a suitable primer. Do not apply with room and surface temperatures below +8 °C. Use the same serial numbers when applying to adjacent areas. One drop = wall height plus 5–10 cm.\nAPPLYING ADHESIVE: (a) Without Aqua Technology, apply sufficient latex adhesive with a paint roller or airless spray gun evenly to the wall over a width of 1–2 sheets. Observe the adhesive manufacturers application notes. This also applies for applications with a wall-papering device. (b) With Aqua Technology, the wall covering comes with a water-activatable adhesive which is already applied to the wall coverings backing. This adhesive can be easily activated by water using the Aqua-Quick device. At normal room temperature/climate (18 °C, 60 %) the drying time is 12–24 hours. When applicating under extreme climatic conditions, the duration can change significantly.\nBUTT-JOINING: Make sure that the edges butt up smoothly where one length joins another. Overlaps in the seam area must be avoided. Our nonwoven wall coverings are suitable for double cutting.\nPRESSING ON AND TRIMMING: Use a (hard plastic) wallpaper spatula and press down firmly across the entire length, smoothing out any air bubbles. Carefully press (the) overlapping fabric into the corners and cut with a sharp knife.\nPAINTING: Apply the paint evenly, once the wall covering has completely dried. Follow the paint manufacturers instructions. The need for further coatings depends on the paint quality, degree of gloss, shade, expected stress, lighting situation and desired surface appearance. With raised fibres: Slight sanding between coatings is possible.", "lang": "en"}, {"value": "Glasvliestapeten werden im Innenbereich an Decken und Wänden in den folgenden Schritten verwendet. Weitere Einzelheiten finden Sie in den technischen Datenblättern. \n\nVORBEREITUNG: Die Untergründe sollten trocken, sauber, glatt und stabil sein. Behandeln Sie saugfähige Untergründe mit einer geeigneten Grundierung vor. Nicht bei Raum- und Oberflächentemperaturen unter +8 °C auftragen. Verwenden Sie beim Auftragen auf benachbarten Flächen dieselben Seriennummern. Eine Bahn = Wandhöhe plus 5-10 cm. \nAUFTRAGEN DES KLEBERS: (a) Bei Glasvliestapeten ohne Aqua Technology tragen Sie ausreichend Dispersionskleber mit einer Farbrolle oder einer Airless-Spritzpistole gleichmäßig in einer Breite von 1-2 Bahnen auf die Wand auf. Beachten Sie die Anwendungshinweise des Klebstoffherstellers. Dies gilt auch für das Verwenden eines Tapeziergeräts. (b) Bei Glasvliestapeten mit Aqua Technology wird der Wandbelag mit einem wasseraktivierbaren Klebstoff geliefert, der bereits auf der Rückseite des Wandbelags aufgebracht ist - dieser Klebstoff kann mit einem 'Aqua-Quick-Gerät' einfach mit Wasser aktiviert werden. Bei normaler Raumtemperatur/Klima (18 °C, 60 %) beträgt die Trocknungszeit 12-24 Stunden. Bei der Verarbeitung unter extremen klimatischen Bedingungen kann sich die Dauer erheblich ändern. \nSTOSSVERKLEBUNG: Die Bahnen auf Stoß verkleben, im Nahtbereich auf eine gute Kontaktierung achten. Überlappungen im Nahtbereich müssen vermieden werden. Die Glasvliestapete eignet sich auch für die Verarbeitung im Doppelnahtschnittverfahren.\nANDRÜCKEN UND ABSCHNEIDEN: Mit Tapezierspachtel bei ausreichendem Druck vollflächig blasenfrei andrücken. Überstände vorsichtig in die Ecken drücken und entlang einer Tapezierspachtel oder eines Beschneidelineals mit einem scharfen Cuttermesser abschneiden.\nBESCHICHTUNG: Farbe nach kompletter Trocknung des Wandbelags gleichmäßig auftragen. Verarbeitungsrichtlinien des Farbherstellers beachten. Die Notwendigkeit weiterer Beschichtungen – ebenfalls erst nach kompletter Trocknung des Wandbelags – ist abhängig von Farbqualität, Glanzgrad, Farbton, erwarteter Beanspruchung, Lichtsituation und erwünschtem Oberflächenbild. Bei aufstehenden Fasern: Leichtes Schleifen zwischen Beschichtungen möglich.", "lang": "de"}]}}, "modellingAndValidation": {"LCIMethodAndAllocation": {"typeOfDataSet": "EPD", "referenceToLCAMethodDetails": [{"shortDescription": [{"value": "Wall coverings.pdf", "lang": "en"}], "type": "source data set", "refObjectId": "b7870c7c-6efe-44c6-a754-ddc51a55f02b"}], "other": {"anies": [{"name": "subType", "value": "specific dataset"}]}}, "dataSourcesTreatmentAndRepresentativeness": {"referenceToDataSource": [{"shortDescription": [{"value": "GaBi Database (all versions)", "lang": "en"}], "type": "source data set", "refObjectId": "28d74cc0-db8b-4d7e-bc44-5f6d56ce0c4a"}, {"shortDescription": [{"value": "GaBi Database Edition 2022, CUP 2022.02", "lang": "en"}], "type": "source data set", "refObjectId": "94f442cb-662e-43ea-a792-4b0a35132e93"}], "useAdviceForDataSet": [{"value": "Scope: \nThis specific EPD document refers to nonwoven glass fibre wall covering produced by Vitrulan Textile Glass GmbH. The production data was recorded in 2021. The production plant is located in Marktschorgast, Germany. \nSystem boundary: \nType of EPD according to EN 15804: \"cradle to gate with options, modules C1–C4, and module D\". The following modules are declared: A1–A3, C, D and additional modules: A4 + A5.\n\nThe following life cycle stages are considered:\n\nProduction - Modules A1-A3\nThe product stage includes:\nRaw material supply (A1): raw glass fleece and coating based on starch besides polymeric materials and inorganic additives\nTransport to the manufacturer (A2)\nManufacturing (A3), including provision of all materials, products and energy, as well as waste processing up to the end-of-waste state.\nConstruction Stage - Modules A4- A5\nThe construction process stage includes:\n\nTransport to the construction site (A4)\nTreatment of packaging material (A5) credits for potential avoided burdens due to energy substitution of electricity and thermal energy generation are declared in module D. Installation losses are also included in this module.\nEnd-of-Life Stage - Modules C1-C4\nMechanical dismantling is considered (C1)\nTransport to EoL (C2)\nDisposal (C4) - landfill of the glass fibre wall covering\n\nBenefits and Loads beyond product system boundary\nNo credits were accounted from the EoL scenario(C4) in module D. The credits in D are solely accounting for the avoided burdens calculated by the inversion of electricity grid mix and thermal energy from natural gas during packaging treatment (A5).", "lang": "en"}, {"value": "Gültigkeitsbereich: \nDieses spezifische EPD-Dokument bezieht sich auf Glasvliestapete für Wand und Decke, die von der Vitrulan Textile Glass GmbH hergestellt wird. Die Produktionsdaten wurden im Jahr 2021 erfasst. Die Produktionsstätte befindet sich in Marktschorgast, Deutschland. \nSystemgrenze: \nTyp der EPD nach EN 15804: \"Cradle to Gate mit Optionen, Module C1-C4 und Modul D\". Die folgenden Module sind deklariert: A1-A3, C, D und zusätzliche Module: A4+A5. Folgende Lebenszyklusphasen werden berücksichtigt: Produktion - Module A1-A3. Die Produktphase umfasst: Rohstoffversorgung (A1): Rohglasvlies und Beschichtung auf Stärkebasis sowie aus polymeren Materialien und anorganischen Zusatzstoffen. Transport zum Hersteller (A2). Herstellung (A3), einschließlich Bereitstellung aller Materialien, Produkte und Energie sowie Abfallverarbeitung bis zum End-of-Waste-Zustand.\nBauphase - Module A4-A5. Die Bauprozessphase umfasst: Transport zur Baustelle (A4), Behandlung des Verpackungsmaterials (A5). Gutschriften für potenziell vermiedene Belastungen durch Energiesubstitution von Strom und thermischer Energieerzeugung werden in Modul D angegeben. Installationsverluste sind ebenfalls in diesem Modul enthalten. End-of-Life-Phase - Module C1-C4. Mechanische Demontage wird berücksichtigt (C1), Transport zum EoL (C2), Entsorgung (C4) - Deponierung der Glasfaserwandverkleidung. Nutzen und Lasten außerhalb der Produktsystemgrenze. Es wurden keine Gutschriften aus dem EoL-Szenario (C4) in Modul D berücksichtigt. Die Gutschriften in D berücksichtigen ausschließlich die vermiedenen Belastungen, die durch die Umkehrung des Stromnetzmixes und der thermischen Energie aus Erdgas bei der Verpackungsbehandlung (A5) berechnet wurden.", "lang": "de"}], "other": {"anies": [{"name": "referenceToOriginalEPD", "value": {"shortDescription": {"value": "Nonwoven glass fibre wall covering.pdf", "defaultValue": "Nonwoven glass fibre wall covering.pdf", "lstrings": [{"lang": "en", "value": "Nonwoven glass fibre wall covering.pdf"}]}, "type": "source data set", "uuid": {"uuid": "2755feef-c680-40cb-9b7c-64b192708200"}, "refObjectId": "2755feef-c680-40cb-9b7c-64b192708200", "resourceURLs": ["https://oekobaudat.de/OEKOBAU.DAT/resource/sources/2755feef-c680-40cb-9b7c-64b192708200/Nonwoven_glass_fibre_wall_covering_17835.pdf?version=00.01.000"]}}]}}, "validation": {"review": [{"referenceToNameOfReviewerAndInstitution": [{"shortDescription": [{"value": "Institut Bauen und Umwelt e. V.", "lang": "en"}], "type": "contact data set", "refObjectId": "d111dbec-b024-4be5-86c5-752d6eb2cf95", "uri": "../contacts/d111dbec-b024-4be5-86c5-752d6eb2cf95.xml"}], "type": "Accredited third party review"}]}, "complianceDeclarations": {"compliance": [{"referenceToComplianceSystem": {"shortDescription": [{"value": "DIN EN 15804+A2", "lang": "en"}], "type": "source data set", "refObjectId": "c0016b33-8cf7-415c-ac6e-deba0d21440d", "uri": "../sources/c0016b33-8cf7-415c-ac6e-deba0d21440d.xml"}}, {"referenceToComplianceSystem": {"shortDescription": [{"value": "ISO 14025", "lang": "en"}], "type": "source data set", "refObjectId": "4f2eb655-6e44-4874-a95a-e28f5442cd4d", "uri": "../sources/4f2eb655-6e44-4874-a95a-e28f5442cd4d.xml"}}]}}, "administrativeInformation": {"commissionerAndGoal": {"referenceToCommissioner": [{"shortDescription": [{"value": "Vitrulan Textile Glass GmbH", "lang": "en"}], "type": "contact data set", "refObjectId": "24e7030f-e356-4c17-9b56-45e80a8f435a", "uri": "../contacts/24e7030f-e356-4c17-9b56-45e80a8f435a.xml"}]}, "dataGenerator": {"referenceToPersonOrEntityGeneratingTheDataSet": [{"shortDescription": [{"value": "Sphera Solutions GmbH", "lang": "en"}], "type": "contact data set", "refObjectId": "623edf96-39d1-4e6f-9892-674c7228546b", "uri": "../contacts/623edf96-39d1-4e6f-9892-674c7228546b.xml"}]}, "dataEntryBy": {"timeStamp": 1704758400000, "referenceToDataSetFormat": [{"shortDescription": [{"value": "ILCD Format", "lang": "en"}], "type": "source data set", "refObjectId": "a97a0155-0234-4b87-b4ce-a45da52f2a40", "uri": "../sources/a97a0155-0234-4b87-b4ce-a45da52f2a40.xml"}, {"shortDescription": [{"value": "EPD-Datenformaterweiterungen v1.2", "lang": "de"}, {"value": "EPD Data Format Extensions v1.2", "lang": "en"}], "type": "source data set", "refObjectId": "a29449fd-aa2f-4de8-b5d7-4b06b43c6fde", "uri": "../sources/a29449fd-aa2f-4de8-b5d7-4b06b43c6fde.xml"}]}, "publicationAndOwnership": {"dataSetVersion": "00.02.000", "referenceToRegistrationAuthority": {"shortDescription": [{"value": "Institut Bauen und Umwelt e. V.", "lang": "en"}], "type": "contact data set", "refObjectId": "d111dbec-b024-4be5-86c5-752d6eb2cf95", "uri": "../contacts/d111dbec-b024-4be5-86c5-752d6eb2cf95.xml"}, "registrationNumber": "EPD-VIT-20230429-CBC1-EN", "referenceToOwnershipOfDataSet": {"shortDescription": [{"value": "Vitrulan Textile Glass GmbH", "lang": "en"}], "type": "contact data set", "refObjectId": "24e7030f-e356-4c17-9b56-45e80a8f435a", "uri": "../contacts/24e7030f-e356-4c17-9b56-45e80a8f435a.xml"}, "copyright": true, "licenseType": "Free of charge for all users and uses", "accessRestrictions": [{"value": "None", "lang": "en"}], "other": {"anies": [{"name": "referenceToPublisher", "value": {"shortDescription": [{"value": "Institut Bauen und Umwelt e. V.", "lang": "en"}], "type": "contact data set", "refObjectId": "d111dbec-b024-4be5-86c5-752d6eb2cf95", "uri": "../contacts/d111dbec-b024-4be5-86c5-752d6eb2cf95.xml"}}]}}}, "exchanges": {"exchange": [{"dataSetInternalID": 0, "referenceToFlowDataSet": {"shortDescription": [{"value": "Nonwoven glass fibre wall covering (Glasvliestapete für Wand und Decke)", "lang": "en"}], "type": "flow data set", "refObjectId": "375c19e5-8995-cbe8-4ccd-3fdf1f49e0fb", "uri": "../flows/375c19e5-8995-cbe8-4ccd-3fdf1f49e0fb.xml"}, "meanAmount": 1.0, "referencesToDataSource": {}, "referenceFlow": true, "resolvedFlowVersion": "00.02.000", "resultingflowAmount": 1.0, "flowProperties": [{"name": [{"lang": "en", "value": "Area"}, {"lang": "de", "value": "Fläche"}], "uuid": "93a60a56-a3c8-19da-a746-0800200c9a66", "referenceFlowProperty": true, "meanValue": 1.0, "referenceUnit": "qm", "unitGroupUUID": "c20a03d7-bd90-4569-bc94-66cfd364dfc8"}], "materialProperties": [{"name": "layer thickness", "value": "3.5E-4", "unit": "m", "unitDescription": "meters"}, {"name": "grammage", "value": "0.124", "unit": "kg/m^2", "unitDescription": "kilograms per square meter"}], "typeOfFlow": "Product flow", "classification": {"classHierarchy": "Beschichtungen / Innenbeschichtungen / Wand- und Deckenbeläge", "name": "OEKOBAU.DAT"}}, {"dataSetInternalID": 1, "referenceToFlowDataSet": {"shortDescription": [{"value": "Renewable primary energy as energy carrier (PERE)", "lang": "en"}, {"value": "Erneuerbare Primärenergie als Energieträger (PERE)", "lang": "de"}], "type": "flow data set", "refObjectId": "20f32be5-0398-4288-9b6d-accddd195317", "uri": "../flows/20f32be5-0398-4288-9b6d-accddd195317.xml"}, "exchange direction": "INPUT", "other": {"anies": [{"name": "referenceToUnitGroupDataSet", "value": {"shortDescription": [{"value": "MJ", "lang": "en"}], "type": "unit group data set", "refObjectId": "93a60a57-a3c8-11da-a746-0800200c9a66", "uri": "../unitgroups/93a60a57-a3c8-11da-a746-0800200c9a66.xml"}}, {"value": "1.89715647319081", "module": "A1-A3"}, {"value": "0.000841362160879548", "module": "A4"}, {"value": "0.480839750588105", "module": "A5"}, {"value": "0.0127961593075539", "module": "C1"}, {"value": "0.00048228915156993", "module": "C2"}, {"value": "0", "module": "C3"}, {"value": "0.00363629910112749", "module": "C4"}, {"value": "-0.0299432968559096", "module": "D"}]}, "resolvedFlowVersion": "38.00.000", "flowProperties": [], "typeOfFlow": "Other flow", "classification": {"classHierarchy": "Quantities", "name": "GaBiCategories"}}, {"dataSetInternalID": 2, "referenceToFlowDataSet": {"shortDescription": [{"value": "Renewable primary energy resources as material utilization (PERM)", "lang": "en"}, {"value": "Erneuerbare Primärenergie zur stofflichen Nutzung (PERM)", "lang": "de"}], "type": "flow data set", "refObjectId": "fb3ec0de-548d-4508-aea5-00b73bf6f702", "uri": "../flows/fb3ec0de-548d-4508-aea5-00b73bf6f702.xml"}, "exchange direction": "INPUT", "other": {"anies": [{"name": "referenceToUnitGroupDataSet", "value": {"shortDescription": [{"value": "MJ", "lang": "en"}], "type": "unit group data set", "refObjectId": "93a60a57-a3c8-11da-a746-0800200c9a66", "uri": "../unitgroups/93a60a57-a3c8-11da-a746-0800200c9a66.xml"}}, {"value": "0.35116001793", "module": "A1-A3"}, {"value": "0", "module": "A4"}, {"value": "-0.35116001793", "module": "A5"}, {"value": "0", "module": "C1"}, {"value": "0", "module": "C2"}, {"value": "0", "module": "C3"}, {"value": "0", "module": "C4"}, {"value": "0", "module": "D"}]}, "resolvedFlowVersion": "38.00.000", "flowProperties": [], "typeOfFlow": "Other flow", "classification": {"classHierarchy": "Quantities", "name": "GaBiCategories"}}, {"dataSetInternalID": 3, "referenceToFlowDataSet": {"shortDescription": [{"value": "Total use of renewable primary energy resources (PERT)", "lang": "en"}, {"value": "Total erneuerbare Primärenergie (PERT)", "lang": "de"}], "type": "flow data set", "refObjectId": "53f97275-fa8a-4cdd-9024-65936002acd0", "uri": "../flows/53f97275-fa8a-4cdd-9024-65936002acd0.xml"}, "exchange direction": "INPUT", "other": {"anies": [{"name": "referenceToUnitGroupDataSet", "value": {"shortDescription": [{"value": "MJ", "lang": "en"}], "type": "unit group data set", "refObjectId": "93a60a57-a3c8-11da-a746-0800200c9a66", "uri": "../unitgroups/93a60a57-a3c8-11da-a746-0800200c9a66.xml"}}, {"value": "2.24831649112081", "module": "A1-A3"}, {"value": "0.000841362160879548", "module": "A4"}, {"value": "0.129679732658104", "module": "A5"}, {"value": "0.0127961593075539", "module": "C1"}, {"value": "0.00048228915156993", "module": "C2"}, {"value": "0", "module": "C3"}, {"value": "0.00363629910112749", "module": "C4"}, {"value": "-0.0299432968559096", "module": "D"}]}, "resolvedFlowVersion": "38.00.000", "flowProperties": [], "typeOfFlow": "Other flow", "classification": {"classHierarchy": "Quantities / Environmental quantities / EPD EN 15804 / LCI indicators", "name": "GaBiCategories"}}, {"dataSetInternalID": 4, "referenceToFlowDataSet": {"shortDescription": [{"value": "Non renewable primary energy as energy carrier (PENRE)", "lang": "en"}, {"value": "Nicht-erneuerbare Primärenergie als Energieträger (PENRE)", "lang": "de"}], "type": "flow data set", "refObjectId": "ac857178-2b45-46ec-892a-a9a4332f0372", "uri": "../flows/ac857178-2b45-46ec-892a-a9a4332f0372.xml"}, "exchange direction": "INPUT", "other": {"anies": [{"name": "referenceToUnitGroupDataSet", "value": {"shortDescription": [{"value": "MJ", "lang": "en"}], "type": "unit group data set", "refObjectId": "93a60a57-a3c8-11da-a746-0800200c9a66", "uri": "../unitgroups/93a60a57-a3c8-11da-a746-0800200c9a66.xml"}}, {"value": "11.1945600993911", "module": "A1-A3"}, {"value": "0.0121872884701021", "module": "A4"}, {"value": "0.696004959982149", "module": "A5"}, {"value": "0.0230519614066706", "module": "C1"}, {"value": "0.00698604868329112", "module": "C2"}, {"value": "0", "module": "C3"}, {"value": "0.0242675081085297", "module": "C4"}, {"value": "-0.108851737195651", "module": "D"}]}, "resolvedFlowVersion": "38.00.000", "flowProperties": [], "typeOfFlow": "Other flow", "classification": {"classHierarchy": "Quantities", "name": "GaBiCategories"}}, {"dataSetInternalID": 5, "referenceToFlowDataSet": {"shortDescription": [{"value": "Non renewable primary energy as material utilization (PENRM)", "lang": "en"}, {"value": "Nicht-erneuerbare Primärenergie zur stofflichen Nutzung (PENRM)", "lang": "de"}], "type": "flow data set", "refObjectId": "1421caa0-679d-4bf4-b282-0eb850ccae27", "uri": "../flows/1421caa0-679d-4bf4-b282-0eb850ccae27.xml"}, "exchange direction": "INPUT", "other": {"anies": [{"name": "referenceToUnitGroupDataSet", "value": {"shortDescription": [{"value": "MJ", "lang": "en"}], "type": "unit group data set", "refObjectId": "93a60a57-a3c8-11da-a746-0800200c9a66", "uri": "../unitgroups/93a60a57-a3c8-11da-a746-0800200c9a66.xml"}}, {"value": "0.047895679", "module": "A1-A3"}, {"value": "0", "module": "A4"}, {"value": "-0.047895679", "module": "A5"}, {"value": "0", "module": "C1"}, {"value": "0", "module": "C2"}, {"value": "0", "module": "C3"}, {"value": "0", "module": "C4"}, {"value": "0", "module": "D"}]}, "resolvedFlowVersion": "38.00.000", "flowProperties": [], "typeOfFlow": "Other flow", "classification": {"classHierarchy": "Quantities", "name": "GaBiCategories"}}, {"dataSetInternalID": 6, "referenceToFlowDataSet": {"shortDescription": [{"value": "Total use of non renewable primary energy resources (PENRT)", "lang": "en"}, {"value": "Total nicht erneuerbare Primärenergie (PENRT)", "lang": "de"}], "type": "flow data set", "refObjectId": "06159210-646b-4c8d-8583-da9b3b95a6c1", "uri": "../flows/06159210-646b-4c8d-8583-da9b3b95a6c1.xml"}, "exchange direction": "INPUT", "other": {"anies": [{"name": "referenceToUnitGroupDataSet", "value": {"shortDescription": [{"value": "MJ", "lang": "en"}], "type": "unit group data set", "refObjectId": "93a60a57-a3c8-11da-a746-0800200c9a66", "uri": "../unitgroups/93a60a57-a3c8-11da-a746-0800200c9a66.xml"}}, {"value": "11.2424557783912", "module": "A1-A3"}, {"value": "0.0121872884701021", "module": "A4"}, {"value": "0.648109280982154", "module": "A5"}, {"value": "0.0230519614066707", "module": "C1"}, {"value": "0.00698604868329113", "module": "C2"}, {"value": "0", "module": "C3"}, {"value": "0.0242675081085298", "module": "C4"}, {"value": "-0.108851737195652", "module": "D"}]}, "resolvedFlowVersion": "38.00.000", "flowProperties": [], "typeOfFlow": "Other flow", "classification": {"classHierarchy": "Quantities / Environmental quantities / EPD EN 15804 / LCI indicators", "name": "GaBiCategories"}}, {"dataSetInternalID": 7, "referenceToFlowDataSet": {"shortDescription": [{"value": "Use of secondary material (SM)", "lang": "en"}, {"value": "Einsatz von Sekundärstoffen (SM)", "lang": "de"}], "type": "flow data set", "refObjectId": "c6a1f35f-2d09-4f54-8dfb-97e502e1ce92", "uri": "../flows/c6a1f35f-2d09-4f54-8dfb-97e502e1ce92.xml"}, "exchange direction": "INPUT", "other": {"anies": [{"name": "referenceToUnitGroupDataSet", "value": {"shortDescription": [{"value": "kg", "lang": "en"}], "type": "unit group data set", "refObjectId": "ad38d542-3fe9-439d-9b95-2f5f7752acaf", "uri": "../unitgroups/ad38d542-3fe9-439d-9b95-2f5f7752acaf.xml"}}, {"value": "0.0105722213362298", "module": "A1-A3"}, {"value": "0", "module": "A4"}, {"value": "0.000597975881449363", "module": "A5"}, {"value": "0", "module": "C1"}, {"value": "0", "module": "C2"}, {"value": "0", "module": "C3"}, {"value": "0", "module": "C4"}, {"value": "0", "module": "D"}]}, "resolvedFlowVersion": "38.00.000", "flowProperties": [], "typeOfFlow": "Other flow", "classification": {"classHierarchy": "Quantities / Environmental quantities / EPD EN 15804 / LCI indicators", "name": "GaBiCategories"}}, {"dataSetInternalID": 8, "referenceToFlowDataSet": {"shortDescription": [{"value": "Use of renewable secondary fuels (RSF)", "lang": "en"}, {"value": "Erneuerbare Sekundärbrennstoffe (RSF)", "lang": "de"}], "type": "flow data set", "refObjectId": "64333088-a55f-4aa2-9a31-c10b07816787", "uri": "../flows/64333088-a55f-4aa2-9a31-c10b07816787.xml"}, "exchange direction": "INPUT", "other": {"anies": [{"name": "referenceToUnitGroupDataSet", "value": {"shortDescription": [{"value": "MJ", "lang": "en"}], "type": "unit group data set", "refObjectId": "93a60a57-a3c8-11da-a746-0800200c9a66", "uri": "../unitgroups/93a60a57-a3c8-11da-a746-0800200c9a66.xml"}}, {"value": "0", "module": "A1-A3"}, {"value": "0", "module": "A4"}, {"value": "0", "module": "A5"}, {"value": "0", "module": "C1"}, {"value": "0", "module": "C2"}, {"value": "0", "module": "C3"}, {"value": "0", "module": "C4"}, {"value": "0", "module": "D"}]}, "resolvedFlowVersion": "38.00.000", "flowProperties": [], "typeOfFlow": "Other flow", "classification": {"classHierarchy": "Quantities / Environmental quantities / EPD EN 15804 / LCI indicators", "name": "GaBiCategories"}}, {"dataSetInternalID": 9, "referenceToFlowDataSet": {"shortDescription": [{"value": "Use of non renewable secondary fuels (NRSF)", "lang": "en"}, {"value": "Nicht erneuerbare Sekundärbrennstoffe (NRSF)", "lang": "de"}], "type": "flow data set", "refObjectId": "89def144-d39a-4287-b86f-efde453ddcb2", "uri": "../flows/89def144-d39a-4287-b86f-efde453ddcb2.xml"}, "exchange direction": "INPUT", "other": {"anies": [{"name": "referenceToUnitGroupDataSet", "value": {"shortDescription": [{"value": "MJ", "lang": "en"}], "type": "unit group data set", "refObjectId": "93a60a57-a3c8-11da-a746-0800200c9a66", "uri": "../unitgroups/93a60a57-a3c8-11da-a746-0800200c9a66.xml"}}, {"value": "0", "module": "A1-A3"}, {"value": "0", "module": "A4"}, {"value": "0", "module": "A5"}, {"value": "0", "module": "C1"}, {"value": "0", "module": "C2"}, {"value": "0", "module": "C3"}, {"value": "0", "module": "C4"}, {"value": "0", "module": "D"}]}, "resolvedFlowVersion": "38.00.000", "flowProperties": [], "typeOfFlow": "Other flow", "classification": {"classHierarchy": "Quantities / Environmental quantities / EPD EN 15804 / LCI indicators", "name": "GaBiCategories"}}, {"dataSetInternalID": 10, "referenceToFlowDataSet": {"shortDescription": [{"value": "Use of net fresh water (FW)", "lang": "en"}, {"value": "Einsatz von Süßwasserressourcen (FW)", "lang": "de"}], "type": "flow data set", "refObjectId": "3cf952c8-f3a4-461d-8c96-96456ca62246", "uri": "../flows/3cf952c8-f3a4-461d-8c96-96456ca62246.xml"}, "exchange direction": "INPUT", "other": {"anies": [{"name": "referenceToUnitGroupDataSet", "value": {"shortDescription": [{"value": "m^3", "lang": "en"}], "type": "unit group data set", "refObjectId": "cd950537-0a98-4044-9ba7-9f9a68d0a504", "uri": "../unitgroups/cd950537-0a98-4044-9ba7-9f9a68d0a504.xml"}}, {"value": "0.00757764111069965", "module": "A1-A3"}, {"value": "9.71923728448375E-07", "module": "A4"}, {"value": "0.000533517748999464", "module": "A5"}, {"value": "1.2206772442765E-05", "module": "C1"}, {"value": "5.57130201688683E-07", "module": "C2"}, {"value": "0", "module": "C3"}, {"value": "6.15725529164645E-06", "module": "C4"}, {"value": "-2.87843053159327E-05", "module": "D"}]}, "resolvedFlowVersion": "38.00.000", "flowProperties": [], "typeOfFlow": "Other flow", "classification": {"classHierarchy": "Quantities / Environmental quantities / EPD EN 15804 / LCI indicators", "name": "GaBiCategories"}}, {"dataSetInternalID": 11, "referenceToFlowDataSet": {"shortDescription": [{"value": "Hazardous waste disposed (HWD)", "lang": "en"}, {"value": "Gefährlicher Abfall zur Deponie (HWD)", "lang": "de"}], "type": "flow data set", "refObjectId": "430f9e0f-59b2-46a0-8e0d-55e0e84948fc", "uri": "../flows/430f9e0f-59b2-46a0-8e0d-55e0e84948fc.xml"}, "exchange direction": "OUTPUT", "other": {"anies": [{"name": "referenceToUnitGroupDataSet", "value": {"shortDescription": [{"value": "kg", "lang": "en"}], "type": "unit group data set", "refObjectId": "ad38d542-3fe9-439d-9b95-2f5f7752acaf", "uri": "../unitgroups/ad38d542-3fe9-439d-9b95-2f5f7752acaf.xml"}}, {"value": "5.06184380138049E-09", "module": "A1-A3"}, {"value": "6.44854042848418E-14", "module": "A4"}, {"value": "2.87341411664782E-10", "module": "A5"}, {"value": "1.99474132824068E-12", "module": "C1"}, {"value": "3.69645942820487E-14", "module": "C2"}, {"value": "0", "module": "C3"}, {"value": "1.24608944048305E-12", "module": "C4"}, {"value": "-1.47279422480468E-11", "module": "D"}]}, "resolvedFlowVersion": "38.00.000", "flowProperties": [], "typeOfFlow": "Other flow", "classification": {"classHierarchy": "Quantities / Environmental quantities / EPD EN 15804 / LCI indicators", "name": "GaBiCategories"}}, {"dataSetInternalID": 12, "referenceToFlowDataSet": {"shortDescription": [{"value": "Non hazardous waste disposed (NHWD)", "lang": "en"}, {"value": "Entsorgter nicht gefährlicher Abfall (NHWD)", "lang": "de"}], "type": "flow data set", "refObjectId": "b29ef66b-e286-4afa-949f-62f1a7b4d7fa", "uri": "../flows/b29ef66b-e286-4afa-949f-62f1a7b4d7fa.xml"}, "exchange direction": "OUTPUT", "other": {"anies": [{"name": "referenceToUnitGroupDataSet", "value": {"shortDescription": [{"value": "kg", "lang": "en"}], "type": "unit group data set", "refObjectId": "ad38d542-3fe9-439d-9b95-2f5f7752acaf", "uri": "../unitgroups/ad38d542-3fe9-439d-9b95-2f5f7752acaf.xml"}}, {"value": "0.0935871979755141", "module": "A1-A3"}, {"value": "1.98561257179627E-06", "module": "A4"}, {"value": "0.013073625398912", "module": "A5"}, {"value": "1.73663658030215E-05", "module": "C1"}, {"value": "1.13820117795303E-06", "module": "C2"}, {"value": "0", "module": "C3"}, {"value": "0.124122054723686", "module": "C4"}, {"value": "-5.50389503947938E-05", "module": "D"}]}, "resolvedFlowVersion": "38.00.000", "flowProperties": [], "typeOfFlow": "Other flow", "classification": {"classHierarchy": "Quantities / Environmental quantities / EPD EN 15804 / LCI indicators", "name": "GaBiCategories"}}, {"dataSetInternalID": 13, "referenceToFlowDataSet": {"shortDescription": [{"value": "Radioactive waste disposed (RWD)", "lang": "en"}, {"value": "Entsorgter radioaktiver Abfall (RWD)", "lang": "de"}], "type": "flow data set", "refObjectId": "3449546e-52ad-4b39-b809-9fb77cea8ff6", "uri": "../flows/3449546e-52ad-4b39-b809-9fb77cea8ff6.xml"}, "exchange direction": "OUTPUT", "other": {"anies": [{"name": "referenceToUnitGroupDataSet", "value": {"shortDescription": [{"value": "kg", "lang": "en"}], "type": "unit group data set", "refObjectId": "ad38d542-3fe9-439d-9b95-2f5f7752acaf", "uri": "../unitgroups/ad38d542-3fe9-439d-9b95-2f5f7752acaf.xml"}}, {"value": "0.000347192757926064", "module": "A1-A3"}, {"value": "2.26231201054806E-08", "module": "A4"}, {"value": "2.0201971756024E-05", "module": "A5"}, {"value": "3.68467074189071E-06", "module": "C1"}, {"value": "1.29681199236852E-08", "module": "C2"}, {"value": "0", "module": "C3"}, {"value": "2.69518962054711E-07", "module": "C4"}, {"value": "-8.58648394931769E-06", "module": "D"}]}, "resolvedFlowVersion": "38.00.000", "flowProperties": [], "typeOfFlow": "Other flow", "classification": {"classHierarchy": "Quantities / Environmental quantities / EPD EN 15804 / LCI indicators", "name": "GaBiCategories"}}, {"dataSetInternalID": 14, "referenceToFlowDataSet": {"shortDescription": [{"value": "Components for re-use (CRU)", "lang": "en"}, {"value": "Komponenten für die Wiederverwendung (CRU)", "lang": "de"}], "type": "flow data set", "refObjectId": "a2b32f97-3fc7-4af2-b209-525bc6426f33", "uri": "../flows/a2b32f97-3fc7-4af2-b209-525bc6426f33.xml"}, "exchange direction": "OUTPUT", "other": {"anies": [{"name": "referenceToUnitGroupDataSet", "value": {"shortDescription": [{"value": "kg", "lang": "en"}], "type": "unit group data set", "refObjectId": "ad38d542-3fe9-439d-9b95-2f5f7752acaf", "uri": "../unitgroups/ad38d542-3fe9-439d-9b95-2f5f7752acaf.xml"}}, {"value": "0", "module": "A1-A3"}, {"value": "0", "module": "A4"}, {"value": "0", "module": "A5"}, {"value": "0", "module": "C1"}, {"value": "0", "module": "C2"}, {"value": "0", "module": "C3"}, {"value": "0", "module": "C4"}, {"value": "0", "module": "D"}]}, "resolvedFlowVersion": "38.00.000", "flowProperties": [], "typeOfFlow": "Other flow", "classification": {"classHierarchy": "Quantities / Environmental quantities / EPD EN 15804 / LCI indicators", "name": "GaBiCategories"}}, {"dataSetInternalID": 15, "referenceToFlowDataSet": {"shortDescription": [{"value": "Materials for recycling (MFR)", "lang": "en"}, {"value": "Stoffe zum Recycling (MFR)", "lang": "de"}], "type": "flow data set", "refObjectId": "d7fe48a5-4103-49c8-9aae-b0b5dfdbd6ae", "uri": "../flows/d7fe48a5-4103-49c8-9aae-b0b5dfdbd6ae.xml"}, "exchange direction": "OUTPUT", "other": {"anies": [{"name": "referenceToUnitGroupDataSet", "value": {"shortDescription": [{"value": "kg", "lang": "en"}], "type": "unit group data set", "refObjectId": "ad38d542-3fe9-439d-9b95-2f5f7752acaf", "uri": "../unitgroups/ad38d542-3fe9-439d-9b95-2f5f7752acaf.xml"}}, {"value": "0", "module": "A1-A3"}, {"value": "0", "module": "A4"}, {"value": "0", "module": "A5"}, {"value": "0", "module": "C1"}, {"value": "0", "module": "C2"}, {"value": "0", "module": "C3"}, {"value": "0", "module": "C4"}, {"value": "0", "module": "D"}]}, "resolvedFlowVersion": "38.00.000", "flowProperties": [], "typeOfFlow": "Other flow", "classification": {"classHierarchy": "Quantities / Environmental quantities / EPD EN 15804 / LCI indicators", "name": "GaBiCategories"}}, {"dataSetInternalID": 16, "referenceToFlowDataSet": {"shortDescription": [{"value": "Materials for energy recovery (MER)", "lang": "en"}, {"value": "Stoffe für die Energierückgewinnung (MER)", "lang": "de"}], "type": "flow data set", "refObjectId": "59a9181c-3aaf-46ee-8b13-2b3723b6e447", "uri": "../flows/59a9181c-3aaf-46ee-8b13-2b3723b6e447.xml"}, "exchange direction": "OUTPUT", "other": {"anies": [{"name": "referenceToUnitGroupDataSet", "value": {"shortDescription": [{"value": "kg", "lang": "en"}], "type": "unit group data set", "refObjectId": "ad38d542-3fe9-439d-9b95-2f5f7752acaf", "uri": "../unitgroups/ad38d542-3fe9-439d-9b95-2f5f7752acaf.xml"}}, {"value": "0", "module": "A1-A3"}, {"value": "0", "module": "A4"}, {"value": "0", "module": "A5"}, {"value": "0", "module": "C1"}, {"value": "0", "module": "C2"}, {"value": "0", "module": "C3"}, {"value": "0", "module": "C4"}, {"value": "0", "module": "D"}]}, "resolvedFlowVersion": "38.00.000", "flowProperties": [], "typeOfFlow": "Other flow", "classification": {"classHierarchy": "Quantities / Environmental quantities / EPD EN 15804 / LCI indicators", "name": "GaBiCategories"}}, {"dataSetInternalID": 17, "referenceToFlowDataSet": {"shortDescription": [{"value": "Exported electrical energy (EEE)", "lang": "en"}, {"value": "Exportierte elektrische Energie (EEE)", "lang": "de"}], "type": "flow data set", "refObjectId": "4da0c987-2b76-40d6-9e9e-82a017aaaf29", "uri": "../flows/4da0c987-2b76-40d6-9e9e-82a017aaaf29.xml"}, "exchange direction": "OUTPUT", "other": {"anies": [{"name": "referenceToUnitGroupDataSet", "value": {"shortDescription": [{"value": "MJ", "lang": "en"}], "type": "unit group data set", "refObjectId": "93a60a57-a3c8-11da-a746-0800200c9a66", "uri": "../unitgroups/93a60a57-a3c8-11da-a746-0800200c9a66.xml"}}, {"value": "0", "module": "A1-A3"}, {"value": "0", "module": "A4"}, {"value": "0.030459792165214", "module": "A5"}, {"value": "0", "module": "C1"}, {"value": "0", "module": "C2"}, {"value": "0", "module": "C3"}, {"value": "0", "module": "C4"}, {"value": "0", "module": "D"}]}, "resolvedFlowVersion": "38.00.000", "flowProperties": [], "typeOfFlow": "Other flow", "classification": {"classHierarchy": "Quantities / Environmental quantities / EPD EN 15804 / LCI indicators", "name": "GaBiCategories"}}, {"dataSetInternalID": 18, "referenceToFlowDataSet": {"shortDescription": [{"value": "Exported thermal energy (EET)", "lang": "en"}, {"value": "Exportierte thermische Energie (EET)", "lang": "de"}], "type": "flow data set", "refObjectId": "98daf38a-7a79-46d3-9a37-2b7bd0955810", "uri": "../flows/98daf38a-7a79-46d3-9a37-2b7bd0955810.xml"}, "exchange direction": "OUTPUT", "other": {"anies": [{"name": "referenceToUnitGroupDataSet", "value": {"shortDescription": [{"value": "MJ", "lang": "en"}], "type": "unit group data set", "refObjectId": "93a60a57-a3c8-11da-a746-0800200c9a66", "uri": "../unitgroups/93a60a57-a3c8-11da-a746-0800200c9a66.xml"}}, {"value": "0", "module": "A1-A3"}, {"value": "0", "module": "A4"}, {"value": "0.0545722635342614", "module": "A5"}, {"value": "0", "module": "C1"}, {"value": "0", "module": "C2"}, {"value": "0", "module": "C3"}, {"value": "0", "module": "C4"}, {"value": "0", "module": "D"}]}, "resolvedFlowVersion": "38.00.000", "flowProperties": [], "typeOfFlow": "Other flow", "classification": {"classHierarchy": "Quantities / Environmental quantities / EPD EN 15804 / LCI indicators", "name": "GaBiCategories"}}]}, "LCIAResults": {"LCIAResult": [{"referenceToLCIAMethodDataSet": {"shortDescription": [{"value": "Global Warming Potential total (GWP-total)", "lang": "en"}, {"value": "Globales Erwärmungspotenzial total (GWP-total)", "lang": "de"}], "type": "LCIA method data set", "refObjectId": "6a37f984-a4b3-458a-a20a-64418c145fa2", "uri": "../lciamethods/6a37f984-a4b3-458a-a20a-64418c145fa2.xml"}, "other": {"anies": [{"name": "referenceToUnitGroupDataSet", "value": {"shortDescription": [{"value": "kg CO_(2) eq", "lang": "en"}], "type": "unit group data set", "refObjectId": "1ebf3012-d0db-4de2-aefd-ef30cedb0be1", "uri": "../unitgroups/1ebf3012-d0db-4de2-aefd-ef30cedb0be1.xml"}}, {"value": "0.510876136943556", "module": "A1-A3"}, {"value": "0.000917465492449603", "module": "A4"}, {"value": "0.0697508572526905", "module": "A5"}, {"value": "0.00128194500959548", "module": "C1"}, {"value": "0.000525635735388967", "module": "C2"}, {"value": "0", "module": "C3"}, {"value": "0.0223870973032108", "module": "C4"}, {"value": "-0.00643205801761934", "module": "D"}]}}, {"referenceToLCIAMethodDataSet": {"shortDescription": [{"value": "Global Warming Potential fossil fuels (GWP-fossil)", "lang": "en"}, {"value": "Globales Erwärmungspotenzial fossil (GWP-fossil)", "lang": "de"}], "type": "LCIA method data set", "refObjectId": "5f635281-343e-44fb-83df-1971b155e6b6", "uri": "../lciamethods/5f635281-343e-44fb-83df-1971b155e6b6.xml"}, "other": {"anies": [{"name": "referenceToUnitGroupDataSet", "value": {"shortDescription": [{"value": "kg CO_(2) eq", "lang": "en"}], "type": "unit group data set", "refObjectId": "1ebf3012-d0db-4de2-aefd-ef30cedb0be1", "uri": "../unitgroups/1ebf3012-d0db-4de2-aefd-ef30cedb0be1.xml"}}, {"value": "0.560623794462922", "module": "A1-A3"}, {"value": "0.000907424262691725", "module": "A4"}, {"value": "0.0362900773329465", "module": "A5"}, {"value": "0.00127023683927303", "module": "C1"}, {"value": "0.000519879859210601", "module": "C2"}, {"value": "0", "module": "C3"}, {"value": "0.00185024757911634", "module": "C4"}, {"value": "-0.00639858235053151", "module": "D"}]}}, {"referenceToLCIAMethodDataSet": {"shortDescription": [{"value": "Global Warming Potential biogenic (GWP-biogenic)", "lang": "en"}, {"value": "Globales Erwärmungspotenzial biogen (GWP-biogenic)", "lang": "de"}], "type": "LCIA method data set", "refObjectId": "2356e1ab-0185-4db5-86e5-16de51c7485c", "uri": "../lciamethods/2356e1ab-0185-4db5-86e5-16de51c7485c.xml"}, "other": {"anies": [{"name": "referenceToUnitGroupDataSet", "value": {"shortDescription": [{"value": "kg CO_(2) eq", "lang": "en"}], "type": "unit group data set", "refObjectId": "1ebf3012-d0db-4de2-aefd-ef30cedb0be1", "uri": "../unitgroups/1ebf3012-d0db-4de2-aefd-ef30cedb0be1.xml"}}, {"value": "-0.0500013373908648", "module": "A1-A3"}, {"value": "3.80985137165221E-06", "module": "A4"}, {"value": "0.0334455608867834", "module": "A5"}, {"value": "1.14395256718522E-05", "module": "C1"}, {"value": "2.18389928810186E-06", "module": "C2"}, {"value": "0", "module": "C3"}, {"value": "0.020533434170405", "module": "C4"}, {"value": "-3.27712862324795E-05", "module": "D"}]}}, {"referenceToLCIAMethodDataSet": {"shortDescription": [{"value": "Global Warming Potential luluc (GWP-luluc)", "lang": "en"}, {"value": "Globales Erwärmungspotenzial luluc (GWP-luluc)", "lang": "de"}], "type": "LCIA method data set", "refObjectId": "4331bbdb-978a-490d-8707-eeb047f01a55", "uri": "../lciamethods/4331bbdb-978a-490d-8707-eeb047f01a55.xml"}, "other": {"anies": [{"name": "referenceToUnitGroupDataSet", "value": {"shortDescription": [{"value": "kg CO_(2) eq", "lang": "en"}], "type": "unit group data set", "refObjectId": "1ebf3012-d0db-4de2-aefd-ef30cedb0be1", "uri": "../unitgroups/1ebf3012-d0db-4de2-aefd-ef30cedb0be1.xml"}}, {"value": "0.000253679871499193", "module": "A1-A3"}, {"value": "6.23137838622578E-06", "module": "A4"}, {"value": "1.52190329606281E-05", "module": "A5"}, {"value": "2.68644650601302E-07", "module": "C1"}, {"value": "3.57197689026365E-06", "module": "C2"}, {"value": "0", "module": "C3"}, {"value": "3.41555368940976E-06", "module": "C4"}, {"value": "-7.04380855344023E-07", "module": "D"}]}}, {"referenceToLCIAMethodDataSet": {"shortDescription": [{"value": "Depletion potential of the stratospheric ozone layer (ODP)", "lang": "en"}, {"value": "Abbau Potential der stratosphärischen Ozonschicht (ODP)", "lang": "de"}], "type": "LCIA method data set", "refObjectId": "b5c629d6-def3-11e6-bf01-fe55135034f3", "uri": "../lciamethods/b5c629d6-def3-11e6-bf01-fe55135034f3.xml"}, "other": {"anies": [{"name": "referenceToUnitGroupDataSet", "value": {"shortDescription": [{"value": "kg CFC11 eq", "lang": "en"}], "type": "unit group data set", "refObjectId": "d9e957c9-7309-4474-bf3a-7777df6c4e5b", "uri": "../unitgroups/d9e957c9-7309-4474-bf3a-7777df6c4e5b.xml"}}, {"value": "2.17170447214941E-12", "module": "A1-A3"}, {"value": "9.08097183931999E-17", "module": "A4"}, {"value": "1.26645919746071E-13", "module": "A5"}, {"value": "1.85948945110762E-14", "module": "C1"}, {"value": "5.20543281770319E-17", "module": "C2"}, {"value": "0", "module": "C3"}, {"value": "4.34688922380881E-15", "module": "C4"}, {"value": "-4.33443266000351E-14", "module": "D"}]}}, {"referenceToLCIAMethodDataSet": {"shortDescription": [{"value": "Acidification potential of land and water (AP)", "lang": "en"}, {"value": "Versauerungspotenzial von Boden und Wasser (AP)", "lang": "de"}], "type": "LCIA method data set", "refObjectId": "b5c611c6-def3-11e6-bf01-fe55135034f3", "uri": "../lciamethods/b5c611c6-def3-11e6-bf01-fe55135034f3.xml"}, "other": {"anies": [{"name": "referenceToUnitGroupDataSet", "value": {"shortDescription": [{"value": "mol H^(+) eq", "lang": "en"}], "type": "unit group data set", "refObjectId": "42e089ac-92bf-4bf2-8ca1-5fc40d18f2ed", "uri": "../unitgroups/42e089ac-92bf-4bf2-8ca1-5fc40d18f2ed.xml"}}, {"value": "0.00219500934404955", "module": "A1-A3"}, {"value": "9.96669975794953E-07", "module": "A4"}, {"value": "0.000133120020143564", "module": "A5"}, {"value": "2.78818988745672E-06", "module": "C1"}, {"value": "6.26650000757217E-07", "module": "C2"}, {"value": "0", "module": "C3"}, {"value": "1.31187542452006E-05", "module": "C4"}, {"value": "-8.42592820981883E-06", "module": "D"}]}}, {"referenceToLCIAMethodDataSet": {"shortDescription": [{"value": "Eutrophication potential aquatic freshwater (EP-freshwater)", "lang": "en"}, {"value": "Eutrophierungspotenzial Süßwasser (EP-freshwater)", "lang": "de"}], "type": "LCIA method data set", "refObjectId": "b53ec18f-7377-4ad3-86eb-cc3f4f276b2b", "uri": "../lciamethods/b53ec18f-7377-4ad3-86eb-cc3f4f276b2b.xml"}, "other": {"anies": [{"name": "referenceToUnitGroupDataSet", "value": {"shortDescription": [{"value": "kg P eq", "lang": "en"}], "type": "unit group data set", "refObjectId": "0429039d-a61d-4590-ba67-aa4a20a810a1", "uri": "../unitgroups/0429039d-a61d-4590-ba67-aa4a20a810a1.xml"}}, {"value": "7.92706584192707E-06", "module": "A1-A3"}, {"value": "3.30341859995956E-09", "module": "A4"}, {"value": "4.49848783081361E-07", "module": "A5"}, {"value": "3.70599290341091E-09", "module": "C1"}, {"value": "1.89359948418563E-09", "module": "C2"}, {"value": "0", "module": "C3"}, {"value": "3.13606976836963E-09", "module": "C4"}, {"value": "-8.81882514253631E-09", "module": "D"}]}}, {"referenceToLCIAMethodDataSet": {"shortDescription": [{"value": "Eutrophication potential aquatic marine (EP-marine)", "lang": "en"}, {"value": "Eutrophierungspotenzial Salzwasser (EP-marine)", "lang": "de"}], "type": "LCIA method data set", "refObjectId": "b5c619fa-def3-11e6-bf01-fe55135034f3", "uri": "../lciamethods/b5c619fa-def3-11e6-bf01-fe55135034f3.xml"}, "other": {"anies": [{"name": "referenceToUnitGroupDataSet", "value": {"shortDescription": [{"value": "kg N eq", "lang": "en"}], "type": "unit group data set", "refObjectId": "d05bb823-ecdf-4686-8c40-bf1d9257859f", "uri": "../unitgroups/d05bb823-ecdf-4686-8c40-bf1d9257859f.xml"}}, {"value": "0.00044059722289129", "module": "A1-A3"}, {"value": "3.14253982674036E-07", "module": "A4"}, {"value": "2.79592545896559E-05", "module": "A5"}, {"value": "6.25650665334781E-07", "module": "C1"}, {"value": "2.08143250796991E-07", "module": "C2"}, {"value": "0", "module": "C3"}, {"value": "3.35438456256565E-06", "module": "C4"}, {"value": "-2.28487063857311E-06", "module": "D"}]}}, {"referenceToLCIAMethodDataSet": {"shortDescription": [{"value": "Eutrophication potential terrestrial (EP-terrestrial)", "lang": "en"}, {"value": "Eutrophierungspotenzial Land (EP-terrestrial)", "lang": "de"}], "type": "LCIA method data set", "refObjectId": "b5c614d2-def3-11e6-bf01-fe55135034f3", "uri": "../lciamethods/b5c614d2-def3-11e6-bf01-fe55135034f3.xml"}, "other": {"anies": [{"name": "referenceToUnitGroupDataSet", "value": {"shortDescription": [{"value": "mol N eq", "lang": "en"}], "type": "unit group data set", "refObjectId": "71b4d617-0ec9-4d3f-b65e-e438940c2401", "uri": "../unitgroups/71b4d617-0ec9-4d3f-b65e-e438940c2401.xml"}}, {"value": "0.00473232355635736", "module": "A1-A3"}, {"value": "3.77575879489589E-06", "module": "A4"}, {"value": "0.000307516544966062", "module": "A5"}, {"value": "6.56377314332477E-06", "module": "C1"}, {"value": "2.48011470211914E-06", "module": "C2"}, {"value": "0", "module": "C3"}, {"value": "3.6858554638701E-05", "module": "C4"}, {"value": "-2.44698742407752E-05", "module": "D"}]}}, {"referenceToLCIAMethodDataSet": {"shortDescription": [{"value": "Formation potential of tropospheric ozone photochemical oxidants (POCP)", "lang": "en"}, {"value": "Bildungspotential für troposphärisches Ozon (POCP)", "lang": "de"}], "type": "LCIA method data set", "refObjectId": "b5c610fe-def3-11e6-bf01-fe55135034f3", "uri": "../lciamethods/b5c610fe-def3-11e6-bf01-fe55135034f3.xml"}, "other": {"anies": [{"name": "referenceToUnitGroupDataSet", "value": {"shortDescription": [{"value": "kg NMVOC eq", "lang": "en"}], "type": "unit group data set", "refObjectId": "d27c25f8-fbc1-44c6-b47b-4adbae4199c6", "uri": "../unitgroups/d27c25f8-fbc1-44c6-b47b-4adbae4199c6.xml"}}, {"value": "0.00131901274731535", "module": "A1-A3"}, {"value": "8.53742935879378E-07", "module": "A4"}, {"value": "8.27974643525669E-05", "module": "A5"}, {"value": "1.6911157000552E-06", "module": "C1"}, {"value": "5.43776359635379E-07", "module": "C2"}, {"value": "0", "module": "C3"}, {"value": "1.01940865007687E-05", "module": "C4"}, {"value": "-6.39421159382296E-06", "module": "D"}]}}, {"referenceToLCIAMethodDataSet": {"shortDescription": [{"value": "Abiotic depletion potential for non fossil resources (ADPE)", "lang": "en"}, {"value": "Potenzial für den abiotischen Abbau nicht fossiler Ressourcen (ADPE)", "lang": "de"}], "type": "LCIA method data set", "refObjectId": "b2ad6494-c78d-11e6-9d9d-cec0c932ce01", "uri": "../lciamethods/b2ad6494-c78d-11e6-9d9d-cec0c932ce01.xml"}, "other": {"anies": [{"name": "referenceToUnitGroupDataSet", "value": {"shortDescription": [{"value": "kg Sb eq", "lang": "en"}], "type": "unit group data set", "refObjectId": "54ccd2d9-a32a-4fc2-923d-f2c8c93e89d4", "uri": "../unitgroups/54ccd2d9-a32a-4fc2-923d-f2c8c93e89d4.xml"}}, {"value": "1.63884394350561E-07", "module": "A1-A3"}, {"value": "9.32046080801353E-11", "module": "A4"}, {"value": "9.3756696716177E-09", "module": "A5"}, {"value": "3.46122265158727E-10", "module": "C1"}, {"value": "5.34271369018837E-11", "module": "C2"}, {"value": "0", "module": "C3"}, {"value": "1.89612884431778E-10", "module": "C4"}, {"value": "-9.66737612273202E-10", "module": "D"}]}}, {"referenceToLCIAMethodDataSet": {"shortDescription": [{"value": "Abiotic depletion potential for fossil resources (ADPF)", "lang": "en"}, {"value": "Potenzial für den abiotischen Abbau fossiler Brennstoffe (ADPF)", "lang": "de"}], "type": "LCIA method data set", "refObjectId": "b2ad6110-c78d-11e6-9d9d-cec0c932ce01", "uri": "../lciamethods/b2ad6110-c78d-11e6-9d9d-cec0c932ce01.xml"}, "other": {"anies": [{"name": "referenceToUnitGroupDataSet", "value": {"shortDescription": [{"value": "MJ", "lang": "en"}], "type": "unit group data set", "refObjectId": "93a60a57-a3c8-11da-a746-0800200c9a66", "uri": "../unitgroups/93a60a57-a3c8-11da-a746-0800200c9a66.xml"}}, {"value": "11.2337439476234", "module": "A1-A3"}, {"value": "0.0121392199927342", "module": "A4"}, {"value": "0.647603683276114", "module": "A5"}, {"value": "0.0230460697316786", "module": "C1"}, {"value": "0.00695849466880729", "module": "C2"}, {"value": "0", "module": "C3"}, {"value": "0.0242379929427583", "module": "C4"}, {"value": "-0.108837066709669", "module": "D"}]}}, {"referenceToLCIAMethodDataSet": {"shortDescription": [{"value": "Water use (WDP)", "lang": "en"}, {"value": "Wassernutzung (WDP)", "lang": "de"}], "type": "LCIA method data set", "refObjectId": "b2ad66ce-c78d-11e6-9d9d-cec0c932ce01", "uri": "../lciamethods/b2ad66ce-c78d-11e6-9d9d-cec0c932ce01.xml"}, "other": {"anies": [{"name": "referenceToUnitGroupDataSet", "value": {"shortDescription": [{"value": "m^(3) world eq deprived", "lang": "en"}], "type": "unit group data set", "refObjectId": "6ae2df01-888e-46c8-b17d-49fa3869b476", "uri": "../unitgroups/6ae2df01-888e-46c8-b17d-49fa3869b476.xml"}}, {"value": "0.183152441022209", "module": "A1-A3"}, {"value": "1.03462457328373E-05", "module": "A4"}, {"value": "0.0148145211016378", "module": "A5"}, {"value": "0.000289716388773703", "module": "C1"}, {"value": "5.93071843307949E-06", "module": "C2"}, {"value": "0", "module": "C3"}, {"value": "0.000202873202855122", "module": "C4"}, {"value": "-0.000682826757659794", "module": "D"}]}}, {"referenceToLCIAMethodDataSet": {"shortDescription": [{"value": "Incidence of disease due to PM emissions (PM)", "lang": "en"}, {"value": "Auftreten von Krankheiten aufgrund von Feinstaubemissionen (PM)", "lang": "de"}], "type": "LCIA method data set", "refObjectId": "b5c602c6-def3-11e6-bf01-fe55135034f3", "uri": "../lciamethods/b5c602c6-def3-11e6-bf01-fe55135034f3.xml"}, "other": {"anies": [{"name": "referenceToUnitGroupDataSet", "value": {"shortDescription": [{"value": "Disease incidence", "lang": "en"}], "type": "unit group data set", "refObjectId": "3883559b-648f-4afc-8ba2-0bd24f3affa3", "uri": "../unitgroups/3883559b-648f-4afc-8ba2-0bd24f3affa3.xml"}}, {"value": "2.27750551212237E-08", "module": "A1-A3"}, {"value": "7.00565829393545E-12", "module": "A4"}, {"value": "1.34126298851664E-09", "module": "A5"}, {"value": "2.31152413979261E-11", "module": "C1"}, {"value": "4.17026167083643E-12", "module": "C2"}, {"value": "0", "module": "C3"}, {"value": "1.61441344908286E-10", "module": "C4"}, {"value": "-6.9794704214645E-11", "module": "D"}]}}, {"referenceToLCIAMethodDataSet": {"shortDescription": [{"value": "Human exposure efficiency relative to U235 (IR)", "lang": "en"}, {"value": "Wirkung durch Exposition des Menschen mit U235 (IR)", "lang": "de"}], "type": "LCIA method data set", "refObjectId": "b5c632be-def3-11e6-bf01-fe55135034f3", "uri": "../lciamethods/b5c632be-def3-11e6-bf01-fe55135034f3.xml"}, "other": {"anies": [{"name": "referenceToUnitGroupDataSet", "value": {"shortDescription": [{"value": "kBq U235 eq", "lang": "en"}], "type": "unit group data set", "refObjectId": "456b05bf-1415-44a9-9993-02452f554c09", "uri": "../unitgroups/456b05bf-1415-44a9-9993-02452f554c09.xml"}}, {"value": "0.0455532437452326", "module": "A1-A3"}, {"value": "3.41597599787233E-06", "module": "A4"}, {"value": "0.00266721119382205", "module": "A5"}, {"value": "0.000624209174233271", "module": "C1"}, {"value": "1.95812010855686E-06", "module": "C2"}, {"value": "0", "module": "C3"}, {"value": "2.99188360455886E-05", "module": "C4"}, {"value": "-0.00145390041236218", "module": "D"}]}}, {"referenceToLCIAMethodDataSet": {"shortDescription": [{"value": "Comparative toxic unit for ecosystems (ETP-fw)", "lang": "en"}, {"value": "Toxizitätsvergleichseinheit für Ökosysteme (ETP-fw)", "lang": "de"}], "type": "LCIA method data set", "refObjectId": "ee1082d1-b0f7-43ca-a1f0-21e2a4a74511", "uri": "../lciamethods/ee1082d1-b0f7-43ca-a1f0-21e2a4a74511.xml"}, "other": {"anies": [{"name": "referenceToUnitGroupDataSet", "value": {"shortDescription": [{"value": "CTUe", "lang": "en"}], "type": "unit group data set", "refObjectId": "aa959ded-f1eb-4efb-9c5c-2d60be36b3e6", "uri": "../unitgroups/aa959ded-f1eb-4efb-9c5c-2d60be36b3e6.xml"}}, {"value": "3.76750594694598", "module": "A1-A3"}, {"value": "0.00860228920447272", "module": "A4"}, {"value": "0.219181434348507", "module": "A5"}, {"value": "0.0100959025361397", "module": "C1"}, {"value": "0.00493115241508774", "module": "C2"}, {"value": "0", "module": "C3"}, {"value": "0.0135783111230393", "module": "C4"}, {"value": "-0.0239358406356351", "module": "D"}]}}, {"referenceToLCIAMethodDataSet": {"shortDescription": [{"value": "Comparative toxic unit for humans (carcinogenic) (HTP-c)", "lang": "en"}, {"value": "Toxizitätsvergleichseinheit für Menschen (krebserregend) (HTP-c)", "lang": "de"}], "type": "LCIA method data set", "refObjectId": "2299222a-bbd8-474f-9d4f-4dd1f18aea7c", "uri": "../lciamethods/2299222a-bbd8-474f-9d4f-4dd1f18aea7c.xml"}, "other": {"anies": [{"name": "referenceToUnitGroupDataSet", "value": {"shortDescription": [{"value": "CTUh", "lang": "en"}], "type": "unit group data set", "refObjectId": "d4c9523e-2d7e-49fd-8469-998f547d3a70", "uri": "../unitgroups/d4c9523e-2d7e-49fd-8469-998f547d3a70.xml"}}, {"value": "1.51673920686386E-09", "module": "A1-A3"}, {"value": "1.77323896936172E-13", "module": "A4"}, {"value": "8.62002786796877E-11", "module": "A5"}, {"value": "2.89974382386596E-13", "module": "C1"}, {"value": "1.0165462464873E-13", "module": "C2"}, {"value": "0", "module": "C3"}, {"value": "2.07249343067163E-12", "module": "C4"}, {"value": "-1.09829456288381E-12", "module": "D"}]}}, {"referenceToLCIAMethodDataSet": {"shortDescription": [{"value": "Comparative toxic unit for humans (noncarcinogenic) (HTP-nc)", "lang": "en"}, {"value": "Toxizitätsvergleichseinheit für Menschen (nicht krebserregend) (HTP-nc)", "lang": "de"}], "type": "LCIA method data set", "refObjectId": "3af763a5-b7a1-48c9-9cee-1f223481fcef", "uri": "../lciamethods/3af763a5-b7a1-48c9-9cee-1f223481fcef.xml"}, "other": {"anies": [{"name": "referenceToUnitGroupDataSet", "value": {"shortDescription": [{"value": "CTUh", "lang": "en"}], "type": "unit group data set", "refObjectId": "d4c9523e-2d7e-49fd-8469-998f547d3a70", "uri": "../unitgroups/d4c9523e-2d7e-49fd-8469-998f547d3a70.xml"}}, {"value": "1.47945331347637E-07", "module": "A1-A3"}, {"value": "9.58369687068947E-12", "module": "A4"}, {"value": "8.39279899023795E-09", "module": "A5"}, {"value": "1.06057172685041E-11", "module": "C1"}, {"value": "5.50775237780878E-12", "module": "C2"}, {"value": "0", "module": "C3"}, {"value": "2.29508223909317E-10", "module": "C4"}, {"value": "-4.21765551933859E-11", "module": "D"}]}}, {"referenceToLCIAMethodDataSet": {"shortDescription": [{"value": "Soil quality index (SQP)", "lang": "en"}, {"value": "Bodenqualitätsindex (SQP)", "lang": "de"}], "type": "LCIA method data set", "refObjectId": "b2ad6890-c78d-11e6-9d9d-cec0c932ce01", "uri": "../lciamethods/b2ad6890-c78d-11e6-9d9d-cec0c932ce01.xml"}, "other": {"anies": [{"name": "referenceToUnitGroupDataSet", "value": {"shortDescription": [{"value": "SQP", "lang": "en"}], "type": "unit group data set", "refObjectId": "f130951c-e67f-4f7f-8dd4-665de3974e18", "uri": "../unitgroups/f130951c-e67f-4f7f-8dd4-665de3974e18.xml"}}, {"value": "9.26000305354532", "module": "A1-A3"}, {"value": "0.00513856263800389", "module": "A4"}, {"value": "0.527295820816475", "module": "A5"}, {"value": "0.00831092954472447", "module": "C1"}, {"value": "0.00294554845725545", "module": "C2"}, {"value": "0", "module": "C3"}, {"value": "0.00504181373794674", "module": "C4"}, {"value": "-0.0194464938044065", "module": "D"}]}}]}, "otherAttributes": {"{http://www.indata.network/EPD/2019}epd-version": "1.2"}, "version": "1.1", "locations": "../ILCDLocations.xml"}