{"processInformation": {"dataSetInformation": {"UUID": "1ba3d2bb-56ca-416d-866c-959f3e83ca77", "name": {"baseName": [{"value": "Electricity grid mix scenario 2030", "lang": "en"}, {"value": "Strom-Mix-Szenario 2030", "lang": "de"}], "functionalUnitFlowProperties": [{"value": "<1kV", "lang": "en"}, {"value": "<1kV", "lang": "de"}]}, "classificationInformation": {"classification": [{"class": [{"value": "Sonstige", "level": 0, "classId": "9"}, {"value": "Energieträger - Bereitstellung frei Verbraucher", "level": 1, "classId": "9.2"}, {"value": "Strom", "level": 2, "classId": "9.2.05"}], "name": "oekobau.dat"}]}, "generalComment": [{"value": "This data set has been modeled according to the European Standard EN 15804+A2 for Sustainable Building. Results are depicted in modules that allow the structured expression of results over the entire life cycle.", "lang": "en"}, {"value": "Dieser Datensatz wurde nach dem European Standard EN 15804+A2 für Nachhaltiges Bauen modelliert. Ergebnisse werden in Modulen abgebildet, die den strukturierten Ausdruck von Ergebnissen über den gesamten Lebenszyklus zulassen.", "lang": "de"}], "other": {"anies": [{"margins": 0, "description": [{"lang": "en"}, {"lang": "de"}]}]}}, "quantitativeReference": {"referenceToReferenceFlow": [100988], "type": "Reference flow(s)"}, "time": {"referenceYear": 2023, "dataSetValidUntil": 2026, "timeRepresentativenessDescription": [{"value": "Annual average", "lang": "en"}, {"value": "Jährlicher Durchschnitt", "lang": "de"}]}, "geography": {"locationOfOperationSupplyOrProduction": {"descriptionOfRestrictions": [{"value": "The data set represents the country specific situation in Germany, focusing on the main technologies, the region specific characteristics and / or import statistics.", "lang": "en"}, {"value": "Der Datensatz bildet die länderspezifische Situation in Deutschland ab. Dabei werden Haupttechnologien, spezifische regionale Charakteristiken und ggf. Importstatistiken berücksichtigt.", "lang": "de"}], "location": "DE"}}, "technology": {"technologyDescriptionAndIncludedProcesses": [{"value": "Future scenario Provision of 1 kWh of electricity free to consumer (year 2030). In the forecast, no progressive political influence on electricity generation was assumed (conservative scenario).\n\nThe detailed composition of the scenario can be found in the attached table. No safety margin was applied to the LCA results.", "lang": "en"}, {"value": "Zukunftsszenario Bereitstellung von 1 kWh Strom frei Verbraucher (Jahr 2030). Bei der Prognose wurde kein progessiver politischer Einfluss auf die Stromerzeugung angenommen (konservatives Szenario).\n\n\n\nDie detaillierte Zusammensetzung des Szenarios kann der angefügten Tabelle entnommen werden. Auf die Ökobilanzergebnisse wurde kein Sicherheitszuschlag angewendet.", "lang": "de"}], "technologicalApplicability": [{"value": "Electrical energy is required for the operation of a wide variety of technical systems, devices and installations in the building context.", "lang": "en"}, {"value": "Elektrische Energie wird für den Betrieb verschiedenster technischer Anlagen, Geräte und Installationen im Gebäudekontext benötigt.", "lang": "de"}], "referenceToTechnologyPictogramme": {"shortDescription": [{"value": "energy_electricity_modelling_of_electricity_consumption_mixes.jpg", "lang": "en"}], "type": "source data set", "refObjectId": "b9c7ef87-b7de-4c20-82ab-dfcc3df8dc3b", "version": "24.01.000", "uri": "../sources/b9c7ef87-b7de-4c20-82ab-dfcc3df8dc3b.xml"}, "referenceToTechnologyFlowDiagrammOrPicture": [{"shortDescription": [{"value": "energy_projection electricity mix de (eu energy trends 2013).jpg", "lang": "en"}], "type": "source data set", "refObjectId": "aeba62ac-2bbe-4478-b784-814f0b2f6d04", "version": "24.01.000", "uri": "../sources/aeba62ac-2bbe-4478-b784-814f0b2f6d04.xml"}]}}, "modellingAndValidation": {"LCIMethodAndAllocation": {"typeOfDataSet": "EPD", "other": {"anies": [{"name": "subType", "value": "generic dataset"}]}}, "dataSourcesTreatmentAndRepresentativeness": {"referenceToDataSource": [{"shortDescription": [{"value": "K.Weissermel, H.- J. Arpe: Industrial organic chemistry", "lang": "en"}], "type": "source data set", "refObjectId": "6de1e618-4960-4b0e-aa2c-7f561a1b6f03", "version": "24.01.000", "uri": "../sources/6de1e618-4960-4b0e-aa2c-7f561a1b6f03.xml"}, {"shortDescription": [{"value": "Copper development association: Overview of Recycled Copper", "lang": "en"}], "type": "source data set", "refObjectId": "2b041bb8-adea-4fab-9e28-8abfe409033a", "version": "24.01.000", "uri": "../sources/2b041bb8-adea-4fab-9e28-8abfe409033a.xml"}, {"shortDescription": [{"value": "Smelter Tech: The Reverberatory Furnace ", "lang": "en"}], "type": "source data set", "refObjectId": "b2012fa6-b2f7-4151-b781-aadfaacf4136", "version": "24.01.000", "uri": "../sources/b2012fa6-b2f7-4151-b781-aadfaacf4136.xml"}, {"shortDescription": [{"value": "Process for the production of a plasticized polyvinyl butyral for gluing a base onto a glazing", "lang": "en"}], "type": "source data set", "refObjectId": "9b8971e3-b693-49f0-a0ef-2353e4cfb60b", "version": "24.01.000", "uri": "../sources/9b8971e3-b693-49f0-a0ef-2353e4cfb60b.xml"}, {"shortDescription": [{"value": "LookChem: Manufacture of 1.12-Dodecanedioic Acid", "lang": "en"}], "type": "source data set", "refObjectId": "2ea4220d-0ba7-4351-b99b-545de2232365", "version": "24.01.000", "uri": "../sources/2ea4220d-0ba7-4351-b99b-545de2232365.xml"}, {"shortDescription": [{"value": "Methods of making cyclododecatriene and", "lang": "en"}], "type": "source data set", "refObjectId": "4a1fd634-a5ff-4bd1-a08e-95750cda3a35", "version": "24.01.000", "uri": "../sources/4a1fd634-a5ff-4bd1-a08e-95750cda3a35.xml"}, {"shortDescription": [{"value": "EPA - Health and Environmental Effects Profile for 2-Chloro-1,3-Butadiene, 1984", "lang": "en"}], "type": "source data set", "refObjectId": "56c9aae6-4e0b-4b66-b898-d59cc485198b", "version": "24.01.000", "uri": "../sources/56c9aae6-4e0b-4b66-b898-d59cc485198b.xml"}, {"shortDescription": [{"value": "Chlorpropanes, Chlorobutanes, and Chlorobutenes: Chapter in Ullmann's, 2011", "lang": "en"}], "type": "source data set", "refObjectId": "7e35dd34-81c9-488b-9a69-2b525bfe2999", "version": "24.01.000", "uri": "../sources/7e35dd34-81c9-488b-9a69-2b525bfe2999.xml"}, {"shortDescription": [{"value": "Chloroprene  - Données technico-économiques sur les substances chimiques en France - 2006", "lang": "en"}], "type": "source data set", "refObjectId": "d54f049a-2ece-4140-ac8d-caa694d1d1e9", "version": "24.01.000", "uri": "../sources/d54f049a-2ece-4140-ac8d-caa694d1d1e9.xml"}, {"shortDescription": [{"value": "Renewables Information 2011", "lang": "en"}], "type": "source data set", "refObjectId": "47b981ff-8e4a-4973-8aab-d88611ff3a06", "version": "24.01.000", "uri": "../sources/47b981ff-8e4a-4973-8aab-d88611ff3a06.xml"}, {"shortDescription": [{"value": "eGrid2012 Version 1.0", "lang": "en"}], "type": "source data set", "refObjectId": "3ebd4e78-289a-4b3a-ba90-1071b2ea1a3e", "version": "24.01.000", "uri": "../sources/3ebd4e78-289a-4b3a-ba90-1071b2ea1a3e.xml"}, {"shortDescription": [{"value": "Update of the Environmental Indicators and Energy Payback Time of CIS Modules in Europe, 2010", "lang": "en"}], "type": "source data set", "refObjectId": "acb3a6c1-d206-46ed-8b68-1067eb388a90", "version": "24.01.000", "uri": "../sources/acb3a6c1-d206-46ed-8b68-1067eb388a90.xml"}, {"shortDescription": [{"value": "Sustainability Evaluation of Solar Energy Systems: LCA Analysis (LCA of Thin Film Technologies)", "lang": "en"}], "type": "source data set", "refObjectId": "e831a684-0b46-4c3a-b754-009dd58883ae", "version": "24.01.000", "uri": "../sources/e831a684-0b46-4c3a-b754-009dd58883ae.xml"}, {"shortDescription": [{"value": "Life Cycle Inventories and Life Cycle Assessments of Photovoltaic Systems, 2011", "lang": "en"}], "type": "source data set", "refObjectId": "58b86392-5559-43b1-9d76-7e7a33134051", "version": "24.01.000", "uri": "../sources/58b86392-5559-43b1-9d76-7e7a33134051.xml"}, {"shortDescription": [{"value": "Environmental Life Cycle Inventory of Crystalline Silicon Photovoltaic System Production, 2006", "lang": "en"}], "type": "source data set", "refObjectId": "6b29835e-9afe-410d-a650-c8eb7cedf7a3", "version": "24.01.000", "uri": "../sources/6b29835e-9afe-410d-a650-c8eb7cedf7a3.xml"}, {"shortDescription": [{"value": "Update of environmental indicators and energy payback time of CdTe PV systems in Europe, 2011", "lang": "en"}], "type": "source data set", "refObjectId": "41603ac1-427a-4b74-a6d2-07124c811a06", "version": "24.01.000", "uri": "../sources/41603ac1-427a-4b74-a6d2-07124c811a06.xml"}, {"shortDescription": [{"value": "Energy payback, life cycle CO2 emissions of the BOS in optimized 3.5 MW PV installation", "lang": "en"}], "type": "source data set", "refObjectId": "db43ce49-69ff-436b-b2ba-0d711ee292d2", "version": "24.01.000", "uri": "../sources/db43ce49-69ff-436b-b2ba-0d711ee292d2.xml"}, {"shortDescription": [{"value": "Methodology Guidelines on Life Cycle Assessment of Photovoltaic Electricity, 2009", "lang": "en"}], "type": "source data set", "refObjectId": "83c23f89-16d9-4687-9fb5-b46e5632c594", "version": "24.01.000", "uri": "../sources/83c23f89-16d9-4687-9fb5-b46e5632c594.xml"}, {"shortDescription": [{"value": "Annual European Union greenhouse gas inventory 1990 - 2008 and inventory report 2010", "lang": "en"}], "type": "source data set", "refObjectId": "d19e0017-9ce6-41f6-80d8-1ddcba714d92", "version": "24.01.000", "uri": "../sources/d19e0017-9ce6-41f6-80d8-1ddcba714d92.xml"}, {"shortDescription": [{"value": "Air pollutant emissions in Finland 1990-2008 Informative Inventory report", "lang": "en"}], "type": "source data set", "refObjectId": "4d0b4cd8-ef1e-4b9f-9cc0-a15164f1f1c6", "version": "24.01.000", "uri": "../sources/4d0b4cd8-ef1e-4b9f-9cc0-a15164f1f1c6.xml"}, {"shortDescription": [{"value": "Air pollutant emissions from stationary installations using bioenergy in the NLs BOLK Phase 2", "lang": "en"}], "type": "source data set", "refObjectId": "63ab79ca-79b8-480a-93ff-23b6e10f3301", "version": "24.01.000", "uri": "../sources/63ab79ca-79b8-480a-93ff-23b6e10f3301.xml"}, {"shortDescription": [{"value": "2da Comunicacion Nacional de la Republica Argentina", "lang": "en"}], "type": "source data set", "refObjectId": "4d9277ae-6882-4704-9da8-d864fe7035a6", "version": "24.01.000", "uri": "../sources/4d9277ae-6882-4704-9da8-d864fe7035a6.xml"}, {"shortDescription": [{"value": "2006 IPCC Guidelines for National Greenhouse Gas Inventories", "lang": "en"}], "type": "source data set", "refObjectId": "676b2a43-4d64-47d3-939d-17361afd74df", "version": "24.01.000", "uri": "../sources/676b2a43-4d64-47d3-939d-17361afd74df.xml"}, {"shortDescription": [{"value": "13. Verordnung zur Durchführung des Bundes-Immissionsschutzgesetzes", "lang": "en"}], "type": "source data set", "refObjectId": "d2743393-5fbd-11db-b0de-0800200c9a66", "version": "24.01.000", "uri": "../sources/d2743393-5fbd-11db-b0de-0800200c9a66.xml"}, {"shortDescription": [{"value": "Auswertung PV-Leistung", "lang": "en"}], "type": "source data set", "refObjectId": "fdf1a71b-fde9-4939-b14e-164ff0f4d094", "version": "24.01.000", "uri": "../sources/fdf1a71b-fde9-4939-b14e-164ff0f4d094.xml"}, {"shortDescription": [{"value": "Austria's National Inventory Report 2010", "lang": "en"}], "type": "source data set", "refObjectId": "c175a776-a82f-4739-a0cf-1ac02966df7a", "version": "24.01.000", "uri": "../sources/c175a776-a82f-4739-a0cf-1ac02966df7a.xml"}, {"shortDescription": [{"value": "Austria's Informative Inventory Report (IIR) 2010", "lang": "en"}], "type": "source data set", "refObjectId": "1f692183-8c45-4d9a-87d0-2cb0cdadaf9c", "version": "24.01.000", "uri": "../sources/1f692183-8c45-4d9a-87d0-2cb0cdadaf9c.xml"}, {"shortDescription": [{"value": "Australian National Greenhouse Accounts (NIR)", "lang": "en"}], "type": "source data set", "refObjectId": "6b02aa13-02c4-4f89-b418-51c46249cd74", "version": "24.01.000", "uri": "../sources/6b02aa13-02c4-4f89-b418-51c46249cd74.xml"}, {"shortDescription": [{"value": "Australian electricity generation report 2008", "lang": "en"}], "type": "source data set", "refObjectId": "13f3c0d9-2cd1-40d6-a887-8132d168ce49", "version": "24.01.000", "uri": "../sources/13f3c0d9-2cd1-40d6-a887-8132d168ce49.xml"}, {"shortDescription": [{"value": "Appendix H: Calorific Value, Price, and Emission Coefficients of Energy Kinds", "lang": "en"}], "type": "source data set", "refObjectId": "af10f2b3-4618-47f0-bae4-57e2ba035a5b", "version": "24.01.000", "uri": "../sources/af10f2b3-4618-47f0-bae4-57e2ba035a5b.xml"}, {"shortDescription": [{"value": "Appendix 17 Thermal values and Emission factors energy.xls GWP conversion factors 2006", "lang": "en"}], "type": "source data set", "refObjectId": "b61ddd50-66c1-4b57-a62b-1b3eff1d5c88", "version": "24.01.000", "uri": "../sources/b61ddd50-66c1-4b57-a62b-1b3eff1d5c88.xml"}, {"shortDescription": [{"value": "Anthropogenic Emissions from Energy Activities in India", "lang": "en"}], "type": "source data set", "refObjectId": "074971c8-93ee-41ec-b368-d04410a29499", "version": "24.01.000", "uri": "../sources/074971c8-93ee-41ec-b368-d04410a29499.xml"}, {"shortDescription": [{"value": "Emission Estimation Technique Manual for Fossil Fuel Electric Power Generation Version 2.3", "lang": "en"}], "type": "source data set", "refObjectId": "45ebaf6b-1827-40ab-afc8-5cdf4adbe55f", "version": "24.01.000", "uri": "../sources/45ebaf6b-1827-40ab-afc8-5cdf4adbe55f.xml"}, {"shortDescription": [{"value": "Emisiones atmosféricas de las centrales eléctricas en América del Norte", "lang": "en"}], "type": "source data set", "refObjectId": "c400ff58-c292-41cf-9b9b-2ae4efe728be", "version": "24.01.000", "uri": "../sources/c400ff58-c292-41cf-9b9b-2ae4efe728be.xml"}, {"shortDescription": [{"value": "EMEP/EEA air pollutant emission inventory guidebook - 2009", "lang": "en"}], "type": "source data set", "refObjectId": "9049ae1c-8dc6-4452-bdda-9a0fd0dabef6", "version": "24.01.000", "uri": "../sources/9049ae1c-8dc6-4452-bdda-9a0fd0dabef6.xml"}, {"shortDescription": [{"value": "EMEP/CORINAIR  Emission Inventory Guidebook - 2006", "lang": "en"}], "type": "source data set", "refObjectId": "ed37667c-d18a-4745-bdc3-2d1907a758c5", "version": "24.01.000", "uri": "../sources/ed37667c-d18a-4745-bdc3-2d1907a758c5.xml"}, {"shortDescription": [{"value": "Electricity Gas Australia", "lang": "en"}], "type": "source data set", "refObjectId": "09f34c8b-3240-4a63-ab33-1aca513c5b0a", "version": "24.01.000", "uri": "../sources/09f34c8b-3240-4a63-ab33-1aca513c5b0a.xml"}, {"shortDescription": [{"value": "Electric Power Industry 2009: Year in Review", "lang": "en"}], "type": "source data set", "refObjectId": "8b23bb67-fbe3-48e4-9191-bdb52c8fbb28", "version": "24.01.000", "uri": "../sources/8b23bb67-fbe3-48e4-9191-bdb52c8fbb28.xml"}, {"shortDescription": [{"value": "Directive 2009/28/EC of the European Parliament and of the Council of 23 April 2009", "lang": "en"}], "type": "source data set", "refObjectId": "f3323ac4-38f6-4bff-95b9-0cc97275e91e", "version": "24.01.000", "uri": "../sources/f3323ac4-38f6-4bff-95b9-0cc97275e91e.xml"}, {"shortDescription": [{"value": "Digest of United Kingdom Energy Statistics 2010", "lang": "en"}], "type": "source data set", "refObjectId": "c524c263-6f87-41a1-9998-10806f915e4f", "version": "24.01.000", "uri": "../sources/c524c263-6f87-41a1-9998-10806f915e4f.xml"}, {"shortDescription": [{"value": "Denmark's National Inventory report 2010", "lang": "en"}], "type": "source data set", "refObjectId": "95fbb395-92f4-4993-b88d-5a4cd3ff5471", "version": "24.01.000", "uri": "../sources/95fbb395-92f4-4993-b88d-5a4cd3ff5471.xml"}, {"shortDescription": [{"value": "Danish Emission inventories for stationary combustion plants", "lang": "en"}], "type": "source data set", "refObjectId": "3b917ad4-fb71-43b1-be0b-806537efbfeb", "version": "24.01.000", "uri": "../sources/3b917ad4-fb71-43b1-be0b-806537efbfeb.xml"}, {"shortDescription": [{"value": "Compilation of Air Pollutant Emission Factors", "lang": "en"}], "type": "source data set", "refObjectId": "02564626-8de7-43b0-b671-8dfa43044be8", "version": "24.01.000", "uri": "../sources/02564626-8de7-43b0-b671-8dfa43044be8.xml"}, {"shortDescription": [{"value": "Climate change - Immision Inventory", "lang": "en"}], "type": "source data set", "refObjectId": "5f5d9711-aa38-4ca5-9c43-0b6737d7c48b", "version": "24.01.000", "uri": "../sources/5f5d9711-aa38-4ca5-9c43-0b6737d7c48b.xml"}, {"shortDescription": [{"value": "BVT - Festlegung in ausgewählten industriellen Bereichen als Beitrag zur Erfüllung der Klimasch...", "lang": "en"}], "type": "source data set", "refObjectId": "d7d8f94e-c30b-47f4-aadb-b64a0134cc33", "version": "24.01.000", "uri": "../sources/d7d8f94e-c30b-47f4-aadb-b64a0134cc33.xml"}, {"shortDescription": [{"value": "Brennstoffe und Verbrennungsrechnung, 2. Auflage", "lang": "en"}], "type": "source data set", "refObjectId": "a719ff4c-3b16-4090-b9bc-aac600d7a690", "version": "24.01.000", "uri": "../sources/a719ff4c-3b16-4090-b9bc-aac600d7a690.xml"}, {"shortDescription": [{"value": "Brennstoffe und Verbrennungsrechnung", "lang": "en"}], "type": "source data set", "refObjectId": "cf5a4784-0372-43d0-a814-a2b52132ff11", "version": "24.01.000", "uri": "../sources/cf5a4784-0372-43d0-a814-a2b52132ff11.xml"}, {"shortDescription": [{"value": "Belgium's Greenhouse Gas Inventory (1990-2008)", "lang": "en"}], "type": "source data set", "refObjectId": "14a1e369-d2e8-4054-a4c9-c20f14be6195", "version": "24.01.000", "uri": "../sources/14a1e369-d2e8-4054-a4c9-c20f14be6195.xml"}, {"shortDescription": [{"value": "Greenhouse Gas Emissions in the Netherlands 1990-2008", "lang": "en"}], "type": "source data set", "refObjectId": "a5806d02-3a7d-4ebc-9edb-d82d4a254625", "version": "24.01.000", "uri": "../sources/a5806d02-3a7d-4ebc-9edb-d82d4a254625.xml"}, {"shortDescription": [{"value": "Greenhouse Gas Emissions in Finland 1990-2008", "lang": "en"}], "type": "source data set", "refObjectId": "952089a6-fdba-406f-ac7f-c0c3b2286a65", "version": "24.01.000", "uri": "../sources/952089a6-fdba-406f-ac7f-c0c3b2286a65.xml"}, {"shortDescription": [{"value": "Greenhouse Gas Emissions in Estonia 1990-2008", "lang": "en"}], "type": "source data set", "refObjectId": "d83bb703-1ab5-4306-b324-c6b61e0951a7", "version": "24.01.000", "uri": "../sources/d83bb703-1ab5-4306-b324-c6b61e0951a7.xml"}, {"shortDescription": [{"value": "Greenhouse Gas Emission in Estonia", "lang": "en"}], "type": "source data set", "refObjectId": "a2bb6096-1c77-46a8-8fe5-59b1b3590c83", "version": "24.01.000", "uri": "../sources/a2bb6096-1c77-46a8-8fe5-59b1b3590c83.xml"}, {"shortDescription": [{"value": "GHG Inventories 2008 - Common Reporting Format (CRF)", "lang": "en"}], "type": "source data set", "refObjectId": "cd6f1cfc-f0f8-4270-aa6d-69bdec0e8a7d", "version": "24.01.000", "uri": "../sources/cd6f1cfc-f0f8-4270-aa6d-69bdec0e8a7d.xml"}, {"shortDescription": [{"value": "Full fuel cycle greenhouse gas emission analysis for proposed Kwinana CCGT power station", "lang": "en"}], "type": "source data set", "refObjectId": "4cf7f11b-29ea-482a-acc2-9014aef4e870", "version": "24.01.000", "uri": "../sources/4cf7f11b-29ea-482a-acc2-9014aef4e870.xml"}, {"shortDescription": [{"value": "Ermittlung und Evaluierung von Emissionsfaktoren für Feuerungsanlagen in Deutschland", "lang": "en"}], "type": "source data set", "refObjectId": "580c3724-d564-4c28-bacd-297a8a10ef60", "version": "24.01.000", "uri": "../sources/580c3724-d564-4c28-bacd-297a8a10ef60.xml"}, {"shortDescription": [{"value": "Erarbeitung der Grundlagen für das BVT - Merkblatt Großfeuerungsanlagen", "lang": "en"}], "type": "source data set", "refObjectId": "8f9004d8-69bc-4bfb-ae2c-ec49304abc8d", "version": "24.01.000", "uri": "../sources/8f9004d8-69bc-4bfb-ae2c-ec49304abc8d.xml"}, {"shortDescription": [{"value": "Environmental Report 2008", "lang": "en"}], "type": "source data set", "refObjectId": "010e303b-7e52-4a01-b176-4ac26f4b7eac", "version": "24.01.000", "uri": "../sources/010e303b-7e52-4a01-b176-4ac26f4b7eac.xml"}, {"shortDescription": [{"value": "Energy Statistics  Imports Electricity", "lang": "en"}], "type": "source data set", "refObjectId": "debe5c14-a3c5-4ae1-8f00-ac91dbdcc12d", "version": "24.01.000", "uri": "../sources/debe5c14-a3c5-4ae1-8f00-ac91dbdcc12d.xml"}, {"shortDescription": [{"value": "Energy Futures and Urban Air Pollution: Challenges for China and the United States", "lang": "en"}], "type": "source data set", "refObjectId": "39c74932-1b36-41ed-9ed7-2e8fc678b95a", "version": "24.01.000", "uri": "../sources/39c74932-1b36-41ed-9ed7-2e8fc678b95a.xml"}, {"shortDescription": [{"value": "Energy Consumption, Energy Savings and Emission Analysis for Industrial Motors", "lang": "en"}], "type": "source data set", "refObjectId": "6961baea-190f-4bc4-9aed-c7231f20f128", "version": "24.01.000", "uri": "../sources/6961baea-190f-4bc4-9aed-c7231f20f128.xml"}, {"shortDescription": [{"value": "Emissoes dos Gases Geradores do Efeito Estufa por Termelctricas no Periodo 2000 a 2020", "lang": "en"}], "type": "source data set", "refObjectId": "1a433db5-054d-4795-adc2-1618b790eca2", "version": "24.01.000", "uri": "../sources/1a433db5-054d-4795-adc2-1618b790eca2.xml"}, {"shortDescription": [{"value": "Emissionsschätzungen für SO2, NO2, NMVOC und NH3 in Deutschland 2000-2020", "lang": "en"}], "type": "source data set", "refObjectId": "78626e1d-4507-4562-8c0d-18d84f8bcfe4", "version": "24.01.000", "uri": "../sources/78626e1d-4507-4562-8c0d-18d84f8bcfe4.xml"}, {"shortDescription": [{"value": "Emissionsfaktoren und Kohlenstoffgehalte", "lang": "en"}], "type": "source data set", "refObjectId": "a648a855-48d6-4dfa-a65f-7ef376c077b0", "version": "24.01.000", "uri": "../sources/a648a855-48d6-4dfa-a65f-7ef376c077b0.xml"}, {"shortDescription": [{"value": "Emissions of greenhouse gases in Iceland from 1990 to 2008", "lang": "en"}], "type": "source data set", "refObjectId": "4300d477-7d2e-46ed-bcc4-226e1877565c", "version": "24.01.000", "uri": "../sources/4300d477-7d2e-46ed-bcc4-226e1877565c.xml"}, {"shortDescription": [{"value": "Evaluation Criteria Investment Proposals (translated from hellenic)", "lang": "en"}], "type": "source data set", "refObjectId": "37800c0d-0dbc-436e-99eb-d3790e3c8d1c", "version": "24.01.000", "uri": "../sources/37800c0d-0dbc-436e-99eb-d3790e3c8d1c.xml"}, {"shortDescription": [{"value": "Greenhouse Gas Emissions Inventory Reports of Spain 1990-2008", "lang": "en"}], "type": "source data set", "refObjectId": "308acd86-30a4-42c9-b68c-6ed6a2931877", "version": "24.01.000", "uri": "../sources/308acd86-30a4-42c9-b68c-6ed6a2931877.xml"}, {"shortDescription": [{"value": "Life Cycle Inventory for Electricity Generation in China", "lang": "en"}], "type": "source data set", "refObjectId": "4560b4c3-bf00-470f-b5ed-140cc4d5a3e7", "version": "24.01.000", "uri": "../sources/4560b4c3-bf00-470f-b5ed-140cc4d5a3e7.xml"}, {"shortDescription": [{"value": "Liechtenstein`s Greenhouse Gas Inventory Report 1990 -2008", "lang": "en"}], "type": "source data set", "refObjectId": "d1047ccd-64b4-4f5e-b403-1887547c55d2", "version": "24.01.000", "uri": "../sources/d1047ccd-64b4-4f5e-b403-1887547c55d2.xml"}, {"shortDescription": [{"value": "Latvia's Informative Inventory 1990- 2008", "lang": "en"}], "type": "source data set", "refObjectId": "2ce438a9-0284-4c06-aaab-9cd27962125d", "version": "24.01.000", "uri": "../sources/2ce438a9-0284-4c06-aaab-9cd27962125d.xml"}, {"shortDescription": [{"value": "Italian Greenhouse Gas Inventory 1990-2008", "lang": "en"}], "type": "source data set", "refObjectId": "7a9db98c-5b25-49b9-ace6-ea693b1e1f6d", "version": "24.01.000", "uri": "../sources/7a9db98c-5b25-49b9-ace6-ea693b1e1f6d.xml"}, {"shortDescription": [{"value": "Ireland - Informative Inventory Report 2010", "lang": "en"}], "type": "source data set", "refObjectId": "20b6f41e-6725-4deb-8d68-dd5cd3447cc0", "version": "24.01.000", "uri": "../sources/20b6f41e-6725-4deb-8d68-dd5cd3447cc0.xml"}, {"shortDescription": [{"value": "Inventory of the U.S. Greenhouse Gas Emissions and Sinks (1990 -2008)", "lang": "en"}], "type": "source data set", "refObjectId": "0508ea86-19b8-4557-ad52-10bc9f73452f", "version": "24.01.000", "uri": "../sources/0508ea86-19b8-4557-ad52-10bc9f73452f.xml"}, {"shortDescription": [{"value": "Inventaire des emissions des grandes installations de combustion en France", "lang": "en"}], "type": "source data set", "refObjectId": "72d46923-91d3-4d2e-8565-0c4be7e8f543", "version": "24.01.000", "uri": "../sources/72d46923-91d3-4d2e-8565-0c4be7e8f543.xml"}, {"shortDescription": [{"value": "Integrated Report 2010", "lang": "en"}], "type": "source data set", "refObjectId": "f99161e2-1e5e-4d6a-8c9a-4164b8ee87b5", "version": "24.01.000", "uri": "../sources/f99161e2-1e5e-4d6a-8c9a-4164b8ee87b5.xml"}, {"shortDescription": [{"value": "Integrated Pollution Prevention and Control (IPPC) - Ref. Doc. on the BAT for Large Combustion Plant", "lang": "en"}], "type": "source data set", "refObjectId": "1a8ea509-dbfd-4ba5-805c-e9ba64d6b0cb", "version": "24.01.000", "uri": "../sources/1a8ea509-dbfd-4ba5-805c-e9ba64d6b0cb.xml"}, {"shortDescription": [{"value": "Integrated Pollution Prevention and Control", "lang": "en"}], "type": "source data set", "refObjectId": "e2e153a9-0d09-4447-a398-f9995717eee9", "version": "24.01.000", "uri": "../sources/e2e153a9-0d09-4447-a398-f9995717eee9.xml"}, {"shortDescription": [{"value": "Informative Inventory Report", "lang": "en"}], "type": "source data set", "refObjectId": "6e2d42b4-545d-4450-b5c4-0963dc5a2e59", "version": "24.01.000", "uri": "../sources/6e2d42b4-545d-4450-b5c4-0963dc5a2e59.xml"}, {"shortDescription": [{"value": "India's Initial National Communication to the United Nations Framework Convention on Climate Change", "lang": "en"}], "type": "source data set", "refObjectId": "8ddabeaf-59ca-45e0-b661-5c29be4427f6", "version": "24.01.000", "uri": "../sources/8ddabeaf-59ca-45e0-b661-5c29be4427f6.xml"}, {"shortDescription": [{"value": "Organisation et methodes des inventaires nationaux des emission atmospheriques en France", "lang": "en"}], "type": "source data set", "refObjectId": "1a1829ef-6948-485d-b545-3b72db17264c", "version": "24.01.000", "uri": "../sources/1a1829ef-6948-485d-b545-3b72db17264c.xml"}, {"shortDescription": [{"value": "NIR pour la France au titre de la convention cadre des Nations Unies sur les changements climatiques", "lang": "en"}], "type": "source data set", "refObjectId": "bbc58da8-15bb-4025-90dc-64ae4caed98f", "version": "24.01.000", "uri": "../sources/bbc58da8-15bb-4025-90dc-64ae4caed98f.xml"}, {"shortDescription": [{"value": "New Zealand's Greenhouse Gas Inventory 1990 - 2007", "lang": "en"}], "type": "source data set", "refObjectId": "516c7b37-100e-4481-9f93-00ed916d4541", "version": "24.01.000", "uri": "../sources/516c7b37-100e-4481-9f93-00ed916d4541.xml"}, {"shortDescription": [{"value": "National Inventory Report for 1985-2008 - Hungary", "lang": "en"}], "type": "source data set", "refObjectId": "ccdc8729-d723-4a89-a1a2-60b6cab0c0bb", "version": "24.01.000", "uri": "../sources/ccdc8729-d723-4a89-a1a2-60b6cab0c0bb.xml"}, {"shortDescription": [{"value": "National Inventory Report 2010 Sweden", "lang": "en"}], "type": "source data set", "refObjectId": "15b19a42-6441-4394-bcda-2e49ff1e0fd4", "version": "24.01.000", "uri": "../sources/15b19a42-6441-4394-bcda-2e49ff1e0fd4.xml"}, {"shortDescription": [{"value": "National Inventory Report 2010 Norway", "lang": "en"}], "type": "source data set", "refObjectId": "4b36b132-4a68-431c-bc8b-45d2f5f21fab", "version": "24.01.000", "uri": "../sources/4b36b132-4a68-431c-bc8b-45d2f5f21fab.xml"}, {"shortDescription": [{"value": "National Inventory Report 2010 for Greenhouse Gas Emissions", "lang": "en"}], "type": "source data set", "refObjectId": "23897ee3-ae1e-4a7b-85ea-5c8906d89269", "version": "24.01.000", "uri": "../sources/23897ee3-ae1e-4a7b-85ea-5c8906d89269.xml"}, {"shortDescription": [{"value": "National Inventory Report 2010", "lang": "en"}], "type": "source data set", "refObjectId": "95d3a90d-512b-4b85-8458-f6a859a33d5a", "version": "24.01.000", "uri": "../sources/95d3a90d-512b-4b85-8458-f6a859a33d5a.xml"}, {"shortDescription": [{"value": "National Inventory Report 2010", "lang": "en"}], "type": "source data set", "refObjectId": "ab9a284c-a89e-4f6a-b507-60e0c0b5b551", "version": "24.01.000", "uri": "../sources/ab9a284c-a89e-4f6a-b507-60e0c0b5b551.xml"}, {"shortDescription": [{"value": "National Inventory Report", "lang": "en"}], "type": "source data set", "refObjectId": "8892c020-5266-4d9e-828f-cdf47015d2bb", "version": "24.01.000", "uri": "../sources/8892c020-5266-4d9e-828f-cdf47015d2bb.xml"}, {"shortDescription": [{"value": "National Greenhouse Gas Inventory Report of the Czech Republic, NIR", "lang": "en"}], "type": "source data set", "refObjectId": "b73a174c-74ad-4949-ae92-8e6f321c46b2", "version": "24.01.000", "uri": "../sources/b73a174c-74ad-4949-ae92-8e6f321c46b2.xml"}, {"shortDescription": [{"value": "National Greenhouse Gas Inventory Report of Japan", "lang": "en"}], "type": "source data set", "refObjectId": "9eeb0e0e-b628-4562-afb5-ddc20f317972", "version": "24.01.000", "uri": "../sources/9eeb0e0e-b628-4562-afb5-ddc20f317972.xml"}, {"shortDescription": [{"value": "National Greenhouse Gas Emission Inventory Report 2009 of the Republic of Lithuania", "lang": "en"}], "type": "source data set", "refObjectId": "44b3c207-ff56-4f71-9045-165718811601", "version": "24.01.000", "uri": "../sources/44b3c207-ff56-4f71-9045-165718811601.xml"}, {"shortDescription": [{"value": "Luxembourg´s National Inventory Report 2010 (1990 -2008)", "lang": "en"}], "type": "source data set", "refObjectId": "ff68e8d0-7dde-4614-ba27-cf5262b7859c", "version": "24.01.000", "uri": "../sources/ff68e8d0-7dde-4614-ba27-cf5262b7859c.xml"}, {"shortDescription": [{"value": "Lithuanians's Informative Inventory 2008", "lang": "en"}], "type": "source data set", "refObjectId": "68dd4a61-7521-4dfc-91fe-13513bb38ca1", "version": "24.01.000", "uri": "../sources/68dd4a61-7521-4dfc-91fe-13513bb38ca1.xml"}, {"shortDescription": [{"value": "Switzerland's Greenhouse Gas Inventory 1990-2008", "lang": "en"}], "type": "source data set", "refObjectId": "555d4c66-852f-4743-a1f6-5a47a5a7dc23", "version": "24.01.000", "uri": "../sources/555d4c66-852f-4743-a1f6-5a47a5a7dc23.xml"}, {"shortDescription": [{"value": "Sumas Energy 2 Generation Facility Air Quality Issue Summary", "lang": "en"}], "type": "source data set", "refObjectId": "ef9503bc-edf6-4910-8e93-933446348e4f", "version": "24.01.000", "uri": "../sources/ef9503bc-edf6-4910-8e93-933446348e4f.xml"}, {"shortDescription": [{"value": "Submission under the UN Framework Convention on Climate Change and under the Kyoto Protocol 2010", "lang": "en"}], "type": "source data set", "refObjectId": "f711df00-97d3-47c4-b180-5594b3ebe201", "version": "24.01.000", "uri": "../sources/f711df00-97d3-47c4-b180-5594b3ebe201.xml"}, {"shortDescription": [{"value": "Slovenia's National Inventory Report 2010", "lang": "en"}], "type": "source data set", "refObjectId": "975b5607-1824-4b62-b16d-cd44b9427522", "version": "24.01.000", "uri": "../sources/975b5607-1824-4b62-b16d-cd44b9427522.xml"}, {"shortDescription": [{"value": "Slovak Republic National Inventory Report 2010", "lang": "en"}], "type": "source data set", "refObjectId": "7ed2df76-c25a-428b-870f-bb116cc4ba12", "version": "24.01.000", "uri": "../sources/7ed2df76-c25a-428b-870f-bb116cc4ba12.xml"}, {"shortDescription": [{"value": "Romania's Greenhouse Gas Inventory 1989-2008", "lang": "en"}], "type": "source data set", "refObjectId": "648eabe1-6171-481e-9385-0aa23ca08a9a", "version": "24.01.000", "uri": "../sources/648eabe1-6171-481e-9385-0aa23ca08a9a.xml"}, {"shortDescription": [{"value": "Romanian Informative Inventory 2008", "lang": "en"}], "type": "source data set", "refObjectId": "fef1f400-2e11-4dbe-88eb-459269290154", "version": "24.01.000", "uri": "../sources/fef1f400-2e11-4dbe-88eb-459269290154.xml"}, {"shortDescription": [{"value": "Richtlinie 2009/28/EG des Europäischen Parlaments und des Rates vom 23. April 2009", "lang": "en"}], "type": "source data set", "refObjectId": "f494c11e-737c-4b1b-a911-1d511177b5e3", "version": "24.01.000", "uri": "../sources/f494c11e-737c-4b1b-a911-1d511177b5e3.xml"}, {"shortDescription": [{"value": "Renewables 2010", "lang": "en"}], "type": "source data set", "refObjectId": "b431a232-fe5b-41c5-87b0-94fdb402a733", "version": "24.01.000", "uri": "../sources/b431a232-fe5b-41c5-87b0-94fdb402a733.xml"}, {"shortDescription": [{"value": "Power Hungry: Reinventing The U.S. Electric Grid", "lang": "en"}], "type": "source data set", "refObjectId": "e8f646de-4e1f-40ab-8294-46f81ad67fd1", "version": "24.01.000", "uri": "../sources/e8f646de-4e1f-40ab-8294-46f81ad67fd1.xml"}, {"shortDescription": [{"value": "Power Connections: Canadian Electricity Trade and Foreign Policy", "lang": "en"}], "type": "source data set", "refObjectId": "15fec28d-cbbc-42a8-aed9-4140a217c74e", "version": "24.01.000", "uri": "../sources/15fec28d-cbbc-42a8-aed9-4140a217c74e.xml"}, {"shortDescription": [{"value": "Portuguese National Inventory Report on Grennhouse Gases, 1990-2008", "lang": "en"}], "type": "source data set", "refObjectId": "a25eb4da-f802-4e7b-b8f9-5db9d9d59fc2", "version": "24.01.000", "uri": "../sources/a25eb4da-f802-4e7b-b8f9-5db9d9d59fc2.xml"}, {"shortDescription": [{"value": "Portuguese Informative Inventory 1990-2008", "lang": "en"}], "type": "source data set", "refObjectId": "0aadf465-cc80-4843-93aa-1d2fc5a16263", "version": "24.01.000", "uri": "../sources/0aadf465-cc80-4843-93aa-1d2fc5a16263.xml"}, {"shortDescription": [{"value": "Poland's Informative Inventory 2010", "lang": "en"}], "type": "source data set", "refObjectId": "2e7f9df2-2d00-4ed3-a366-001dc03e43db", "version": "24.01.000", "uri": "../sources/2e7f9df2-2d00-4ed3-a366-001dc03e43db.xml"}, {"shortDescription": [{"value": "Verhaltenes Lächeln auf langen Gesichtern", "lang": "en"}], "type": "source data set", "refObjectId": "71fd4cb6-d468-4dca-8b65-b5b35ad6f80c", "version": "24.01.000", "uri": "../sources/71fd4cb6-d468-4dca-8b65-b5b35ad6f80c.xml"}, {"shortDescription": [{"value": "UK Greenhouse gas inventory, 1990 to 2008", "lang": "en"}], "type": "source data set", "refObjectId": "34a298be-4daa-457f-bd8f-075755d1d42d", "version": "24.01.000", "uri": "../sources/34a298be-4daa-457f-bd8f-075755d1d42d.xml"}, {"shortDescription": [{"value": "Turkey Greenhouse gas Inventory, 1990 to 2008", "lang": "en"}], "type": "source data set", "refObjectId": "6c59444d-2cf1-426d-9df7-93e60364c955", "version": "24.01.000", "uri": "../sources/6c59444d-2cf1-426d-9df7-93e60364c955.xml"}, {"shortDescription": [{"value": "The European Pollutant Release and Transfer Register", "lang": "en"}], "type": "source data set", "refObjectId": "68570e54-3d75-4c1f-b88d-df2a66c2ba30", "version": "24.01.000", "uri": "../sources/68570e54-3d75-4c1f-b88d-df2a66c2ba30.xml"}, {"shortDescription": [{"value": "The CEA Mercury program", "lang": "en"}], "type": "source data set", "refObjectId": "3b65ee48-c719-40f4-ab73-7f0383584712", "version": "24.01.000", "uri": "../sources/3b65ee48-c719-40f4-ab73-7f0383584712.xml"}, {"shortDescription": [{"value": "Telefonische Recherche - Preis Kraftwerksnebenprodukte", "lang": "en"}], "type": "source data set", "refObjectId": "cbede9c2-03b5-457c-a947-6e944f9d39fc", "version": "24.01.000", "uri": "../sources/cbede9c2-03b5-457c-a947-6e944f9d39fc.xml"}, {"shortDescription": [{"value": "EU Energy Trends to 2050", "lang": "en"}], "type": "source data set", "refObjectId": "fd4d74a3-6fe7-4227-9d91-83bcc4fbd80b", "version": "24.01.000", "uri": "../sources/fd4d74a3-6fe7-4227-9d91-83bcc4fbd80b.xml"}, {"shortDescription": [{"value": "Plant-by-Plant emissions reported under LCP directive ", "lang": "en"}], "type": "source data set", "refObjectId": "4ba1c4d7-d4cd-4dbd-9d52-d66e65917097", "version": "24.01.000", "uri": "../sources/4ba1c4d7-d4cd-4dbd-9d52-d66e65917097.xml"}, {"shortDescription": [{"value": "The European offshore wind industry - key trends and statistics 2014", "lang": "en"}], "type": "source data set", "refObjectId": "f0a58cb7-9486-4458-a6a5-4dbef32d871b", "version": "24.01.000", "uri": "../sources/f0a58cb7-9486-4458-a6a5-4dbef32d871b.xml"}, {"shortDescription": [{"value": "China Electric Power Yearbook 2015", "lang": "en"}], "type": "source data set", "refObjectId": "3875965d-fb85-4dc4-94ef-3372b30d7ef9", "version": "24.01.000", "uri": "../sources/3875965d-fb85-4dc4-94ef-3372b30d7ef9.xml"}, {"shortDescription": [{"value": "Wind in power 2016 - European statistics  ", "lang": "en"}], "type": "source data set", "refObjectId": "038ede2d-0650-4acf-89c4-623cad30bbb9", "version": "24.01.000", "uri": "../sources/038ede2d-0650-4acf-89c4-623cad30bbb9.xml"}, {"shortDescription": [{"value": "The European offshore wind industry - key trends and statistics 2015", "lang": "en"}], "type": "source data set", "refObjectId": "d5cfdcc8-52ec-4fdb-8180-4150014ed370", "version": "24.01.000", "uri": "../sources/d5cfdcc8-52ec-4fdb-8180-4150014ed370.xml"}, {"shortDescription": [{"value": "IEA Wind - 2016 Annual report   ", "lang": "en"}], "type": "source data set", "refObjectId": "2593f5d7-97c7-415c-8b5e-035d7178abce", "version": "24.01.000", "uri": "../sources/2593f5d7-97c7-415c-8b5e-035d7178abce.xml"}, {"shortDescription": [{"value": "Statistical Yearbook 2015", "lang": "en"}], "type": "source data set", "refObjectId": "888c15fe-6986-4434-a7e2-39f2b06d0d8e", "version": "24.01.000", "uri": "../sources/888c15fe-6986-4434-a7e2-39f2b06d0d8e.xml"}, {"shortDescription": [{"value": "Energy Balances of OECD Countries 2017", "lang": "en"}], "type": "source data set", "refObjectId": "931e99ab-e2b5-4667-bfd6-d8517f702997", "version": "24.01.000", "uri": "../sources/931e99ab-e2b5-4667-bfd6-d8517f702997.xml"}, {"shortDescription": [{"value": "Energy Statistics of OECD Countries 2017", "lang": "en"}], "type": "source data set", "refObjectId": "fc9d620f-c3b9-46b6-a592-099cdede9eca", "version": "24.01.000", "uri": "../sources/fc9d620f-c3b9-46b6-a592-099cdede9eca.xml"}, {"shortDescription": [{"value": "Energy Balances of Non-OECD Countries 2017 ", "lang": "en"}], "type": "source data set", "refObjectId": "cf73d907-7766-432e-84f7-73bde6bd0e18", "version": "24.01.000", "uri": "../sources/cf73d907-7766-432e-84f7-73bde6bd0e18.xml"}, {"shortDescription": [{"value": "Energy Statistics of Non-OECD Countries 2017", "lang": "en"}], "type": "source data set", "refObjectId": "df41463a-39bb-4787-a194-c676ba6f8523", "version": "24.01.000", "uri": "../sources/df41463a-39bb-4787-a194-c676ba6f8523.xml"}, {"shortDescription": [{"value": "World Energy Statistics 2017", "lang": "en"}], "type": "source data set", "refObjectId": "f8733bf1-8713-445d-9f5c-511452ed6e9c", "version": "24.01.000", "uri": "../sources/f8733bf1-8713-445d-9f5c-511452ed6e9c.xml"}, {"shortDescription": [{"value": "Electricity Information 2017", "lang": "en"}], "type": "source data set", "refObjectId": "f3bbd3d5-6143-400c-ba0c-4d36b745ef9d", "version": "24.01.000", "uri": "../sources/f3bbd3d5-6143-400c-ba0c-4d36b745ef9d.xml"}, {"shortDescription": [{"value": "Bruttostromerzeugung in Deutschland ab 1990 nach Energieträgern ", "lang": "en"}], "type": "source data set", "refObjectId": "5da9b82b-f76e-43fd-89de-6719d195eee0", "version": "24.01.000", "uri": "../sources/5da9b82b-f76e-43fd-89de-6719d195eee0.xml"}, {"shortDescription": [{"value": "Sphera Managed LCA Content Databases (all versions)", "lang": "en"}], "type": "source data set", "refObjectId": "28d74cc0-db8b-4d7e-bc44-5f6d56ce0c4a", "version": "00.03.002", "uri": "../sources/28d74cc0-db8b-4d7e-bc44-5f6d56ce0c4a.xml"}, {"shortDescription": [{"value": "Documentation of data quality management", "lang": "en"}], "type": "source data set", "refObjectId": "e3bd9bbf-2c3c-42aa-8892-fd13f1065ca5", "version": "24.01.000", "uri": "../sources/e3bd9bbf-2c3c-42aa-8892-fd13f1065ca5.xml"}, {"shortDescription": [{"value": "GaBi Database Edition 2021, CUP2021.01", "lang": "en"}], "type": "source data set", "refObjectId": "1cece811-7501-44d4-8067-9259bd5cb835", "version": "00.01.000", "uri": "../sources/1cece811-7501-44d4-8067-9259bd5cb835.xml"}], "useAdviceForDataSet": [{"value": "This data set refers to the production of 1kWh of electrical energy. The dataset is used to estimate future environmental impacts associated with the provision of electrical energy.                                                                                          \n\nThe dataset represents a scenario calculated based on the EU Reference Scenario 2016 - Energy, Transport and GHG Emissions - Trends to 2050 published by the European Commission in 2016.\nThe national or regional specific electricity consumption mix is provided by the conversion of the different energy carriers to electricity and imports from neighbouring countries, as illustrated in the figure \"\"Projection Electricity Mix\"\".\nThe electricity is either produced in energy carrier specific power plants and/or combined heat and power plants (CHP). Also considered are the national and regional specific technology standards of the power plants in regard to efficiency, firing technology, flue-gas desulphurisation, NOx removal and de-dusting. The electricity provided by non-combustible renewable energy sources also considers the national or regional situation, such as solar radiation (photovoltaic), annual full load hours (wind power), and share of hydro power stations by type (run-of-river, storage and pumped storage).\nThe fossil power plant models combine emission data from literature with calculated values for non-measured emissions e.g. organics or heavy metals. For the emissions CO2, SO2, NOx, CO, CH4, N2O, NMVOC and particulate matter (PM) measured/calculated data are used, taken from national inventory reports, emission inventory data bases, utility companies and other sources. The calculation of other emissions within the models are based on energy carrier properties, transfer coefficients and power plant thermodynamics representing the applied flue gas treatment technologies and standards (flue gas desulphurisation, dust filter etc.). Combustion residues from solid fuels, such as gypsum, bottom ash or fly ash are assumed  to be reused e.g. in construction work. Waste treatment for these substances is therefore not considered. Radioactive emissions from ashes are not considered in the coal power plant model.\nThe energy carrier supply considers the whole supply chain of the energy carrier from exploration, production, processing and transport of the fuels to the power plants. The supply chain is modelled in specific national / regional energy carrier consumption mixes (i.e. domestic production and imports), and considers national / regional average energy carrier properties (e.g. elemental composition and energy content).\nThe electricity grid mix includes imported electricity from neighbouring countries, transmission / distribution losses of low or medium voltage electricity supply and the own use of electricity by energy producers (own consumption of power plants, and \"other\" own consumption e.g. due to pumped storage hydro power etc.). The logic of modelling the electricity consumption mix is represented in the flow diagram \"Modelling of Electricity Consumption Mixes\".", "lang": "en"}, {"value": "Dieser Datensatz bezieht sich auf die Herstellung von 1kWh elektrischer Energie. \n\nDer Datensatz dient zur Abschätzung zukünftiger Umweltlasten in Verbindung mit der Bereitstellung elektrischer Energie.\n\nDer Datensatz stellt ein Szenario dar, das auf Grundlage des von der Europäischen Kommission im Jahr 2016 veröffentlichten \"EU Reference Scenario 2016  Energy, Transport and GHG Emissions  Trends to 2050\" berechnet wurde.\n\n\nDer landes- bzw. regionalspezifische Stromverbrauchsmix ergibt sich aus der Umwandlung der unterschiedlichen Energieträger in Strom und Importen aus den Nachbarländern.\n\n\nDer Strom wird entweder in energieträgerspezifischen Kraftwerken und/oder Blockheizkraftwerken (BHKW) erzeugt. Berücksichtigt werden auch die bundes- und regionalspezifischen Technologiestandards der Kraftwerke hinsichtlich Wirkungsgrad, Feuerungstechnik, Rauchgasentschwefelung, NOx-Entfernung und Entstaubung. Die Strombereitstellung aus nicht brennbaren erneuerbaren Energiequellen berücksichtigt auch die nationalen bzw. regionalen Gegebenheiten wie Sonneneinstrahlung (Photovoltaik), jährliche Volllaststunden (Windkraft) und Wasserkraftanteil nach Art (Laufwasser, Speicher und Pumpspeicher).\nDie fossilen Kraftwerksmodelle kombinieren Emissionsdaten aus der Literatur mit berechneten Werten für nicht gemessene Emissionen, z. organische Stoffe oder Schwermetalle. Für die Emissionen CO2, SO2, NOx, CO, CH4, N2O, NMVOC und Feinstaub (PM) werden gemessene/berechnete Daten verwendet, die aus nationalen Inventarberichten, Emissionsinventardatenbanken, Versorgungsunternehmen und anderen Quellen stammen. Die Berechnung anderer Emissionen innerhalb der Modelle basiert auf Energieträgereigenschaften, Übertragungskoeffizienten und Kraftwerksthermodynamik, die die angewandten Rauchgasreinigungstechnologien und -standards (Rauchgasentschwefelung, Staubfilter usw.) darstellen. Es wird davon ausgegangen, dass Verbrennungsrückstände aus festen Brennstoffen wie Gips, Bodenasche oder Flugasche in der Bauwirtschaft verwendet werden. Eine Abfallbehandlung für diese Stoffe wird daher nicht berücksichtigt. Radioaktive Emissionen aus Asche werden im Kohlekraftwerksmodell nicht berücksichtigt.\nDie Energieträgerversorgung betrachtet die gesamte Lieferkette des Energieträgers von der Exploration, Produktion, Verarbeitung und dem Transport der Brennstoffe bis zu den Kraftwerken. Die Lieferkette wird in spezifischen nationalen/regionalen Energieträgerverbrauchsmixen (d. h. inländische Produktion und Importe) modelliert und berücksichtigt nationale/regionale durchschnittliche Energieträgereigenschaften (z. B. Elementzusammensetzung und Energiegehalt).\nDer Stromnetzmix umfasst importierten Strom aus Nachbarländern, Übertragungs-/Verteilungsverluste der Nieder- oder Mittelspannungsstromversorgung und den Eigenverbrauch von Strom durch Energieerzeuger (Eigenverbrauch von Kraftwerken und \"sonstiger\" Eigenverbrauch z.B. durch Pumpspeicherkraftwerke Strom usw.). Die Logik der Modellierung des Stromverbrauchsmixes ist im Flussdiagramm \"Modellierung von Stromverbrauchsmixen\" dargestellt.", "lang": "de"}]}, "validation": {"review": [{"referenceToNameOfReviewerAndInstitution": [{"shortDescription": [{"value": "Sphera Solutions GmbH", "lang": "en"}], "type": "contact data set", "refObjectId": "d7fa0337-f279-430d-becf-7f3111a85010", "version": "24.01.000", "uri": "../contacts/d7fa0337-f279-430d-becf-7f3111a85010.xml"}], "type": "Dependent internal review"}, {"referenceToNameOfReviewerAndInstitution": [{"shortDescription": [{"value": "Sphera Product Sustainability user forum", "lang": "en"}], "type": "contact data set", "refObjectId": "8f1306f0-7b83-4f36-a537-aa83f0498266", "version": "24.01.000", "uri": "../contacts/8f1306f0-7b83-4f36-a537-aa83f0498266.xml"}], "type": "Independent external review"}]}, "complianceDeclarations": {"compliance": [{"referenceToComplianceSystem": {"shortDescription": [{"value": "EN 15804+A2 (EF 3.1)", "lang": "de"}, {"value": "EN 15804+A2 (EF 3.1)", "lang": "en"}], "type": "source data set", "refObjectId": "d4aa3ec7-b1d7-4a4a-a6cb-37af88dcc902", "version": "00.01.000", "uri": "../sources/d4aa3ec7-b1d7-4a4a-a6cb-37af88dcc902.xml"}, "approvalOfOverallCompliance": "Fully compliant"}]}}, "administrativeInformation": {"dataGenerator": {"referenceToPersonOrEntityGeneratingTheDataSet": [{"shortDescription": [{"value": "Sphera Solutions GmbH", "lang": "en"}], "type": "contact data set", "refObjectId": "d7fa0337-f279-430d-becf-7f3111a85010", "version": "24.01.000", "uri": "../contacts/d7fa0337-f279-430d-becf-7f3111a85010.xml"}]}, "dataEntryBy": {"timeStamp": 1718121675000, "referenceToDataSetFormat": [{"shortDescription": [{"value": "ILCD format 1.1", "lang": "de"}, {"value": "ILCD format 1.1", "lang": "en"}], "type": "source data set", "refObjectId": "a97a0155-0234-4b87-b4ce-a45da52f2a40", "version": "01.00.000", "uri": "../sources/a97a0155-0234-4b87-b4ce-a45da52f2a40.xml"}, {"shortDescription": [{"value": "EPD-Datenformaterweiterungen v1.2", "lang": "de"}, {"value": "EPD Data Format Extensions v1.2", "lang": "en"}], "type": "source data set", "refObjectId": "a29449fd-aa2f-4de8-b5d7-4b06b43c6fde", "version": "00.01.000", "uri": "../sources/a29449fd-aa2f-4de8-b5d7-4b06b43c6fde.xml"}], "referenceToPersonOrEntityEnteringTheData": {"shortDescription": [{"value": "Sphera Solutions GmbH", "lang": "en"}], "type": "contact data set", "refObjectId": "d7fa0337-f279-430d-becf-7f3111a85010", "version": "24.01.000", "uri": "../contacts/d7fa0337-f279-430d-becf-7f3111a85010.xml"}}, "publicationAndOwnership": {"dataSetVersion": "20.24.070", "referenceToPrecedingDataSetVersion": [{"shortDescription": [{"value": "Electricity grid mix scenario 2030", "lang": "en"}], "type": "process data set", "refObjectId": "e8e73ef6-ce7c-4c9a-8709-b8573e039b9f", "uri": "https://www.oekobaudat.de/OEKOBAU.DAT/resource/processes/e8e73ef6-ce7c-4c9a-8709-b8573e039b9f?version=20.23.050"}], "referenceToRegistrationAuthority": {"shortDescription": [{"value": "Sphera Solutions GmbH", "lang": "en"}], "type": "contact data set", "refObjectId": "d7fa0337-f279-430d-becf-7f3111a85010", "version": "24.01.000", "uri": "../contacts/d7fa0337-f279-430d-becf-7f3111a85010.xml"}, "referenceToOwnershipOfDataSet": {"shortDescription": [{"value": "Sphera Solutions GmbH", "lang": "en"}], "type": "contact data set", "refObjectId": "d7fa0337-f279-430d-becf-7f3111a85010", "version": "24.01.000", "uri": "../contacts/d7fa0337-f279-430d-becf-7f3111a85010.xml"}, "copyright": true, "licenseType": "Free of charge for all users and uses", "accessRestrictions": [{"value": "The license conditions as stated on https://www.oekobaudat.de/apply.", "lang": "en"}, {"value": "Es gelten die Lizenzbedingungen wie sie auf https://www.oekobaudat.de/ genannt sind.", "lang": "de"}], "other": {"anies": [{"name": "referenceToPublisher", "value": {"shortDescription": [{"value": "BBSR", "lang": "en"}], "type": "contact data set", "refObjectId": "f11651e0-7877-11e3-981f-0800200c9a66", "version": "00.01.000", "uri": "../contacts/f11651e0-7877-11e3-981f-0800200c9a66.xml"}}]}}}, "exchanges": {"exchange": [{"dataSetInternalID": 100988, "referenceToFlowDataSet": {"shortDescription": [{"value": "Electricity grid mix scenario 2030", "lang": "en"}, {"value": "Strom-Mix-Szenario 2030", "lang": "de"}], "type": "flow data set", "refObjectId": "890a70b7-b677-4e2a-8a1b-7d017e0a10ae", "version": "24.01.000", "uri": "../flows/890a70b7-b677-4e2a-8a1b-7d017e0a10ae.xml"}, "meanAmount": 3.6, "referenceFlow": true, "resultingflowAmount": 3.6, "flowProperties": [{"name": [{"lang": "en", "value": "Net calorific value"}, {"lang": "de", "value": "Unterer Heizwert"}], "uuid": "93a60a56-a3c8-11da-a746-0800200c9a66", "referenceFlowProperty": true, "meanValue": 1.0, "referenceUnit": "MJ", "unitGroupUUID": "93a60a57-a3c8-11da-a746-0800200c9a66"}], "typeOfFlow": "Product flow", "classification": {"classHierarchy": "Valuable substances / Energy carrier / Electric power", "name": "GaBiCategories"}}, {"dataSetInternalID": 100989, "referenceToFlowDataSet": {"shortDescription": [{"value": "Use of renewable primary energy as energy carrier (PERE)", "lang": "en"}, {"value": "Erneuerbare Primärenergie als Energieträger (PERE)", "lang": "de"}], "type": "flow data set", "refObjectId": "20f32be5-0398-4288-9b6d-accddd195317", "version": "24.01.000", "uri": "../flows/20f32be5-0398-4288-9b6d-accddd195317.xml"}, "exchange direction": "INPUT", "other": {"anies": [{"value": "8.34051872819316", "module": "B6"}, {"name": "referenceToUnitGroupDataSet", "value": {"shortDescription": [{"value": "MJ", "lang": "en"}], "type": "unit group data set", "refObjectId": "93a60a57-a3c8-11da-a746-0800200c9a66", "version": "03.00.000", "uri": "../unitgroups/93a60a57-a3c8-11da-a746-0800200c9a66.xml"}}]}, "resolvedFlowVersion": "38.00.000", "flowProperties": [], "typeOfFlow": "Other flow", "classification": {"classHierarchy": "Quantities", "name": "GaBiCategories"}}, {"dataSetInternalID": 100990, "referenceToFlowDataSet": {"shortDescription": [{"value": "Use of renewable primary energy resources used as raw materials (PERM)", "lang": "en"}, {"value": "Erneuerbare Primärenergie zur stofflichen Nutzung (PERM)", "lang": "de"}], "type": "flow data set", "refObjectId": "fb3ec0de-548d-4508-aea5-00b73bf6f702", "version": "24.01.000", "uri": "../flows/fb3ec0de-548d-4508-aea5-00b73bf6f702.xml"}, "exchange direction": "INPUT", "other": {"anies": [{"value": "0", "module": "B6"}, {"name": "referenceToUnitGroupDataSet", "value": {"shortDescription": [{"value": "MJ", "lang": "en"}], "type": "unit group data set", "refObjectId": "93a60a57-a3c8-11da-a746-0800200c9a66", "version": "03.00.000", "uri": "../unitgroups/93a60a57-a3c8-11da-a746-0800200c9a66.xml"}}]}, "resolvedFlowVersion": "38.00.000", "flowProperties": [], "typeOfFlow": "Other flow", "classification": {"classHierarchy": "Quantities", "name": "GaBiCategories"}}, {"dataSetInternalID": 100991, "referenceToFlowDataSet": {"shortDescription": [{"value": "Total use of renewable primary energy (PERT)", "lang": "en"}, {"value": "Total erneuerbare Primärenergie (PERT)", "lang": "de"}], "type": "flow data set", "refObjectId": "53f97275-fa8a-4cdd-9024-65936002acd0", "version": "24.01.000", "uri": "../flows/53f97275-fa8a-4cdd-9024-65936002acd0.xml"}, "exchange direction": "INPUT", "other": {"anies": [{"value": "8.34051872819316", "module": "B6"}, {"name": "referenceToUnitGroupDataSet", "value": {"shortDescription": [{"value": "MJ", "lang": "en"}], "type": "unit group data set", "refObjectId": "93a60a57-a3c8-11da-a746-0800200c9a66", "version": "03.00.000", "uri": "../unitgroups/93a60a57-a3c8-11da-a746-0800200c9a66.xml"}}]}, "resolvedFlowVersion": "38.00.000", "flowProperties": [], "typeOfFlow": "Other flow", "classification": {"classHierarchy": "Quantities / Environmental quantities / EPD EN 15804 / LCI indicators", "name": "GaBiCategories"}}, {"dataSetInternalID": 100992, "referenceToFlowDataSet": {"shortDescription": [{"value": "Use of non renewable primary energy as energy carrier (PENRE)", "lang": "en"}, {"value": "Nicht-erneuerbare Primärenergie als Energieträger (PENRE)", "lang": "de"}], "type": "flow data set", "refObjectId": "ac857178-2b45-46ec-892a-a9a4332f0372", "version": "24.01.000", "uri": "../flows/ac857178-2b45-46ec-892a-a9a4332f0372.xml"}, "exchange direction": "INPUT", "other": {"anies": [{"value": "3.76324377730189", "module": "B6"}, {"name": "referenceToUnitGroupDataSet", "value": {"shortDescription": [{"value": "MJ", "lang": "en"}], "type": "unit group data set", "refObjectId": "93a60a57-a3c8-11da-a746-0800200c9a66", "version": "03.00.000", "uri": "../unitgroups/93a60a57-a3c8-11da-a746-0800200c9a66.xml"}}]}, "resolvedFlowVersion": "38.00.000", "flowProperties": [], "typeOfFlow": "Other flow", "classification": {"classHierarchy": "Quantities", "name": "GaBiCategories"}}, {"dataSetInternalID": 100993, "referenceToFlowDataSet": {"shortDescription": [{"value": "Use of non renewable primary energy resources used as raw materials (PENRM)", "lang": "en"}, {"value": "Nicht-erneuerbare Primärenergie zur stofflichen Nutzung (PENRM)", "lang": "de"}], "type": "flow data set", "refObjectId": "1421caa0-679d-4bf4-b282-0eb850ccae27", "version": "24.01.000", "uri": "../flows/1421caa0-679d-4bf4-b282-0eb850ccae27.xml"}, "exchange direction": "INPUT", "other": {"anies": [{"value": "0", "module": "B6"}, {"name": "referenceToUnitGroupDataSet", "value": {"shortDescription": [{"value": "MJ", "lang": "en"}], "type": "unit group data set", "refObjectId": "93a60a57-a3c8-11da-a746-0800200c9a66", "version": "03.00.000", "uri": "../unitgroups/93a60a57-a3c8-11da-a746-0800200c9a66.xml"}}]}, "resolvedFlowVersion": "38.00.000", "flowProperties": [], "typeOfFlow": "Other flow", "classification": {"classHierarchy": "Quantities", "name": "GaBiCategories"}}, {"dataSetInternalID": 100994, "referenceToFlowDataSet": {"shortDescription": [{"value": "Total use of non renewable primary energy resource (PENRT)", "lang": "en"}, {"value": "Total nicht-erneuerbare Primärenergie (PENRT)", "lang": "de"}], "type": "flow data set", "refObjectId": "06159210-646b-4c8d-8583-da9b3b95a6c1", "version": "24.01.000", "uri": "../flows/06159210-646b-4c8d-8583-da9b3b95a6c1.xml"}, "exchange direction": "INPUT", "other": {"anies": [{"value": "3.76324377730189", "module": "B6"}, {"name": "referenceToUnitGroupDataSet", "value": {"shortDescription": [{"value": "MJ", "lang": "en"}], "type": "unit group data set", "refObjectId": "93a60a57-a3c8-11da-a746-0800200c9a66", "version": "03.00.000", "uri": "../unitgroups/93a60a57-a3c8-11da-a746-0800200c9a66.xml"}}]}, "resolvedFlowVersion": "38.00.000", "flowProperties": [], "typeOfFlow": "Other flow", "classification": {"classHierarchy": "Quantities / Environmental quantities / EPD EN 15804 / LCI indicators", "name": "GaBiCategories"}}, {"dataSetInternalID": 100995, "referenceToFlowDataSet": {"shortDescription": [{"value": "Use of secondary material (SM)", "lang": "en"}, {"value": "Einsatz von Sekundärstoffen (SM)", "lang": "de"}], "type": "flow data set", "refObjectId": "c6a1f35f-2d09-4f54-8dfb-97e502e1ce92", "version": "24.01.000", "uri": "../flows/c6a1f35f-2d09-4f54-8dfb-97e502e1ce92.xml"}, "exchange direction": "INPUT", "other": {"anies": [{"value": "0", "module": "B6"}, {"name": "referenceToUnitGroupDataSet", "value": {"shortDescription": [{"value": "kg", "lang": "en"}], "type": "unit group data set", "refObjectId": "93a60a57-a4c8-11da-a746-0800200c9a66", "version": "03.00.000", "uri": "../unitgroups/93a60a57-a4c8-11da-a746-0800200c9a66.xml"}}]}, "resolvedFlowVersion": "38.00.000", "flowProperties": [], "typeOfFlow": "Other flow", "classification": {"classHierarchy": "Quantities / Environmental quantities / EPD EN 15804 / LCI indicators", "name": "GaBiCategories"}}, {"dataSetInternalID": 100996, "referenceToFlowDataSet": {"shortDescription": [{"value": "Use of renewable secondary fuels (SF)", "lang": "en"}, {"value": "Erneuerbare Sekundärbrennstoffe (SF)", "lang": "de"}], "type": "flow data set", "refObjectId": "64333088-a55f-4aa2-9a31-c10b07816787", "version": "24.01.000", "uri": "../flows/64333088-a55f-4aa2-9a31-c10b07816787.xml"}, "exchange direction": "INPUT", "other": {"anies": [{"value": "0", "module": "B6"}, {"name": "referenceToUnitGroupDataSet", "value": {"shortDescription": [{"value": "MJ", "lang": "en"}], "type": "unit group data set", "refObjectId": "93a60a57-a3c8-11da-a746-0800200c9a66", "version": "03.00.000", "uri": "../unitgroups/93a60a57-a3c8-11da-a746-0800200c9a66.xml"}}]}, "resolvedFlowVersion": "38.00.000", "flowProperties": [], "typeOfFlow": "Other flow", "classification": {"classHierarchy": "Quantities / Environmental quantities / EPD EN 15804 / LCI indicators", "name": "GaBiCategories"}}, {"dataSetInternalID": 100997, "referenceToFlowDataSet": {"shortDescription": [{"value": "Use of non renewable secondary fuels (NRSF)", "lang": "en"}, {"value": "Nicht erneuerbare Sekundärbrennstoffe (NRSF)", "lang": "de"}], "type": "flow data set", "refObjectId": "89def144-d39a-4287-b86f-efde453ddcb2", "version": "24.01.000", "uri": "../flows/89def144-d39a-4287-b86f-efde453ddcb2.xml"}, "exchange direction": "INPUT", "other": {"anies": [{"value": "0", "module": "B6"}, {"name": "referenceToUnitGroupDataSet", "value": {"shortDescription": [{"value": "MJ", "lang": "en"}], "type": "unit group data set", "refObjectId": "93a60a57-a3c8-11da-a746-0800200c9a66", "version": "03.00.000", "uri": "../unitgroups/93a60a57-a3c8-11da-a746-0800200c9a66.xml"}}]}, "resolvedFlowVersion": "38.00.000", "flowProperties": [], "typeOfFlow": "Other flow", "classification": {"classHierarchy": "Quantities / Environmental quantities / EPD EN 15804 / LCI indicators", "name": "GaBiCategories"}}, {"dataSetInternalID": 100998, "referenceToFlowDataSet": {"shortDescription": [{"value": "Net use of fresh water (FW)", "lang": "en"}, {"value": "Nettoeinsatz von Süßwasserressourcen (FW)", "lang": "de"}], "type": "flow data set", "refObjectId": "3cf952c8-f3a4-461d-8c96-96456ca62246", "version": "24.01.000", "uri": "../flows/3cf952c8-f3a4-461d-8c96-96456ca62246.xml"}, "exchange direction": "INPUT", "other": {"anies": [{"value": "0.00139449191711561", "module": "B6"}, {"name": "referenceToUnitGroupDataSet", "value": {"shortDescription": [{"value": "m3", "lang": "en"}], "type": "unit group data set", "refObjectId": "93a60a57-a3c8-12da-a746-0800200c9a66", "version": "03.00.000", "uri": "../unitgroups/93a60a57-a3c8-12da-a746-0800200c9a66.xml"}}]}, "resolvedFlowVersion": "38.00.000", "flowProperties": [], "typeOfFlow": "Other flow", "classification": {"classHierarchy": "Quantities / Environmental quantities / EPD EN 15804 / LCI indicators", "name": "GaBiCategories"}}, {"dataSetInternalID": 100999, "referenceToFlowDataSet": {"shortDescription": [{"value": "Hazardous waste disposed (HWD)", "lang": "en"}, {"value": "Gefährlicher Abfall zur Deponie (HWD)", "lang": "de"}], "type": "flow data set", "refObjectId": "430f9e0f-59b2-46a0-8e0d-55e0e84948fc", "version": "24.01.000", "uri": "../flows/430f9e0f-59b2-46a0-8e0d-55e0e84948fc.xml"}, "exchange direction": "OUTPUT", "other": {"anies": [{"value": "2.30878941324806E-8", "module": "B6"}, {"name": "referenceToUnitGroupDataSet", "value": {"shortDescription": [{"value": "kg", "lang": "en"}], "type": "unit group data set", "refObjectId": "93a60a57-a4c8-11da-a746-0800200c9a66", "version": "03.00.000", "uri": "../unitgroups/93a60a57-a4c8-11da-a746-0800200c9a66.xml"}}]}, "resolvedFlowVersion": "38.00.000", "flowProperties": [], "typeOfFlow": "Other flow", "classification": {"classHierarchy": "Quantities / Environmental quantities / EPD EN 15804 / LCI indicators", "name": "GaBiCategories"}}, {"dataSetInternalID": 101000, "referenceToFlowDataSet": {"shortDescription": [{"value": "Non harzardous waste disposed (NHWD)", "lang": "en"}, {"value": "Entsorgter nicht gefährlicher Abfall (NHWD)", "lang": "de"}], "type": "flow data set", "refObjectId": "b29ef66b-e286-4afa-949f-62f1a7b4d7fa", "version": "24.01.000", "uri": "../flows/b29ef66b-e286-4afa-949f-62f1a7b4d7fa.xml"}, "exchange direction": "OUTPUT", "other": {"anies": [{"value": "0.00595369670666214", "module": "B6"}, {"name": "referenceToUnitGroupDataSet", "value": {"shortDescription": [{"value": "kg", "lang": "en"}], "type": "unit group data set", "refObjectId": "93a60a57-a4c8-11da-a746-0800200c9a66", "version": "03.00.000", "uri": "../unitgroups/93a60a57-a4c8-11da-a746-0800200c9a66.xml"}}]}, "resolvedFlowVersion": "38.00.000", "flowProperties": [], "typeOfFlow": "Other flow", "classification": {"classHierarchy": "Quantities / Environmental quantities / EPD EN 15804 / LCI indicators", "name": "GaBiCategories"}}, {"dataSetInternalID": 101001, "referenceToFlowDataSet": {"shortDescription": [{"value": "Radioactive waste disposed (RWD)", "lang": "en"}, {"value": "Entsorgter radioaktiver Abfall (RWD)", "lang": "de"}], "type": "flow data set", "refObjectId": "3449546e-52ad-4b39-b809-9fb77cea8ff6", "version": "24.01.000", "uri": "../flows/3449546e-52ad-4b39-b809-9fb77cea8ff6.xml"}, "exchange direction": "OUTPUT", "other": {"anies": [{"value": "7.23600231944274E-5", "module": "B6"}, {"name": "referenceToUnitGroupDataSet", "value": {"shortDescription": [{"value": "kg", "lang": "en"}], "type": "unit group data set", "refObjectId": "93a60a57-a4c8-11da-a746-0800200c9a66", "version": "03.00.000", "uri": "../unitgroups/93a60a57-a4c8-11da-a746-0800200c9a66.xml"}}]}, "resolvedFlowVersion": "38.00.000", "flowProperties": [], "typeOfFlow": "Other flow", "classification": {"classHierarchy": "Quantities / Environmental quantities / EPD EN 15804 / LCI indicators", "name": "GaBiCategories"}}, {"dataSetInternalID": 101002, "referenceToFlowDataSet": {"shortDescription": [{"value": "Components for re-use (CRU)", "lang": "en"}, {"value": "Komponenten für die Wiederverwendung (CRU)", "lang": "de"}], "type": "flow data set", "refObjectId": "a2b32f97-3fc7-4af2-b209-525bc6426f33", "version": "24.01.000", "uri": "../flows/a2b32f97-3fc7-4af2-b209-525bc6426f33.xml"}, "exchange direction": "OUTPUT", "other": {"anies": [{"value": "0", "module": "B6"}, {"name": "referenceToUnitGroupDataSet", "value": {"shortDescription": [{"value": "kg", "lang": "en"}], "type": "unit group data set", "refObjectId": "93a60a57-a4c8-11da-a746-0800200c9a66", "version": "03.00.000", "uri": "../unitgroups/93a60a57-a4c8-11da-a746-0800200c9a66.xml"}}]}, "resolvedFlowVersion": "38.00.000", "flowProperties": [], "typeOfFlow": "Other flow", "classification": {"classHierarchy": "Quantities / Environmental quantities / EPD EN 15804 / LCI indicators", "name": "GaBiCategories"}}, {"dataSetInternalID": 101003, "referenceToFlowDataSet": {"shortDescription": [{"value": "Materials for recycling  (MFR)", "lang": "en"}, {"value": "Stoffe zum Recycling (MFR)", "lang": "de"}], "type": "flow data set", "refObjectId": "d7fe48a5-4103-49c8-9aae-b0b5dfdbd6ae", "version": "24.01.000", "uri": "../flows/d7fe48a5-4103-49c8-9aae-b0b5dfdbd6ae.xml"}, "exchange direction": "OUTPUT", "other": {"anies": [{"value": "0", "module": "B6"}, {"name": "referenceToUnitGroupDataSet", "value": {"shortDescription": [{"value": "kg", "lang": "en"}], "type": "unit group data set", "refObjectId": "93a60a57-a4c8-11da-a746-0800200c9a66", "version": "03.00.000", "uri": "../unitgroups/93a60a57-a4c8-11da-a746-0800200c9a66.xml"}}]}, "resolvedFlowVersion": "38.00.000", "flowProperties": [], "typeOfFlow": "Other flow", "classification": {"classHierarchy": "Quantities / Environmental quantities / EPD EN 15804 / LCI indicators", "name": "GaBiCategories"}}, {"dataSetInternalID": 101004, "referenceToFlowDataSet": {"shortDescription": [{"value": "Materials for energy recovery (MER)", "lang": "en"}, {"value": "Stoffe für die Energierückgewinnung (MER)", "lang": "de"}], "type": "flow data set", "refObjectId": "59a9181c-3aaf-46ee-8b13-2b3723b6e447", "version": "24.01.000", "uri": "../flows/59a9181c-3aaf-46ee-8b13-2b3723b6e447.xml"}, "exchange direction": "OUTPUT", "other": {"anies": [{"value": "0", "module": "B6"}, {"name": "referenceToUnitGroupDataSet", "value": {"shortDescription": [{"value": "kg", "lang": "en"}], "type": "unit group data set", "refObjectId": "93a60a57-a4c8-11da-a746-0800200c9a66", "version": "03.00.000", "uri": "../unitgroups/93a60a57-a4c8-11da-a746-0800200c9a66.xml"}}]}, "resolvedFlowVersion": "38.00.000", "flowProperties": [], "typeOfFlow": "Other flow", "classification": {"classHierarchy": "Quantities / Environmental quantities / EPD EN 15804 / LCI indicators", "name": "GaBiCategories"}}, {"dataSetInternalID": 101005, "referenceToFlowDataSet": {"shortDescription": [{"value": "Exported electrical energy (EEE)", "lang": "en"}, {"value": "Exportierte elektrische Energie (EEE)", "lang": "de"}], "type": "flow data set", "refObjectId": "4da0c987-2b76-40d6-9e9e-82a017aaaf29", "version": "24.01.000", "uri": "../flows/4da0c987-2b76-40d6-9e9e-82a017aaaf29.xml"}, "exchange direction": "OUTPUT", "other": {"anies": [{"value": "0", "module": "B6"}, {"name": "referenceToUnitGroupDataSet", "value": {"shortDescription": [{"value": "MJ", "lang": "en"}], "type": "unit group data set", "refObjectId": "93a60a57-a3c8-11da-a746-0800200c9a66", "version": "03.00.000", "uri": "../unitgroups/93a60a57-a3c8-11da-a746-0800200c9a66.xml"}}]}, "resolvedFlowVersion": "38.00.000", "flowProperties": [], "typeOfFlow": "Other flow", "classification": {"classHierarchy": "Quantities / Environmental quantities / EPD EN 15804 / LCI indicators", "name": "GaBiCategories"}}, {"dataSetInternalID": 101006, "referenceToFlowDataSet": {"shortDescription": [{"value": "Exported thermal energy (EET)", "lang": "en"}, {"value": "Exportierte thermische Energie (EET)", "lang": "de"}], "type": "flow data set", "refObjectId": "98daf38a-7a79-46d3-9a37-2b7bd0955810", "version": "24.01.000", "uri": "../flows/98daf38a-7a79-46d3-9a37-2b7bd0955810.xml"}, "exchange direction": "OUTPUT", "other": {"anies": [{"value": "0", "module": "B6"}, {"name": "referenceToUnitGroupDataSet", "value": {"shortDescription": [{"value": "MJ", "lang": "en"}], "type": "unit group data set", "refObjectId": "93a60a57-a3c8-11da-a746-0800200c9a66", "version": "03.00.000", "uri": "../unitgroups/93a60a57-a3c8-11da-a746-0800200c9a66.xml"}}]}, "resolvedFlowVersion": "38.00.000", "flowProperties": [], "typeOfFlow": "Other flow", "classification": {"classHierarchy": "Quantities / Environmental quantities / EPD EN 15804 / LCI indicators", "name": "GaBiCategories"}}]}, "LCIAResults": {"LCIAResult": [{"referenceToLCIAMethodDataSet": {"shortDescription": [{"value": "Climate change", "lang": "en"}, {"value": "Globales Erwärmungspotenzial - total (GWP-total)", "lang": "de"}], "type": "LCIA method data set", "refObjectId": "a7ea142a-9749-11ed-a8fc-0242ac120002", "version": "24.01.000", "uri": "../lciamethods/a7ea142a-9749-11ed-a8fc-0242ac120002.xml"}, "other": {"anies": [{"value": "0.35947617231963", "module": "B6"}, {"name": "referenceToUnitGroupDataSet", "value": {"shortDescription": [{"value": "kg CO2 eq.", "lang": "en"}], "type": "unit group data set", "refObjectId": "1ebf3012-d0db-4de2-aefd-ef30cedb0be1", "version": "25.00.000", "uri": "../unitgroups/1ebf3012-d0db-4de2-aefd-ef30cedb0be1.xml"}}]}}, {"referenceToLCIAMethodDataSet": {"shortDescription": [{"value": "Climate change-Fossil", "lang": "en"}, {"value": "Globales Erwärmungspotenzial - fossil (GWP-fossil)", "lang": "de"}], "type": "LCIA method data set", "refObjectId": "a7ea19c0-9749-11ed-a8fc-0242ac120002", "version": "24.01.000", "uri": "../lciamethods/a7ea19c0-9749-11ed-a8fc-0242ac120002.xml"}, "other": {"anies": [{"value": "0.355295019835595", "module": "B6"}, {"name": "referenceToUnitGroupDataSet", "value": {"shortDescription": [{"value": "kg CO2 eq.", "lang": "en"}], "type": "unit group data set", "refObjectId": "1ebf3012-d0db-4de2-aefd-ef30cedb0be1", "version": "25.00.000", "uri": "../unitgroups/1ebf3012-d0db-4de2-aefd-ef30cedb0be1.xml"}}]}}, {"referenceToLCIAMethodDataSet": {"shortDescription": [{"value": "Climate change-Biogenic", "lang": "en"}, {"value": "Globales Erwärmungspotenzial - biogen (GWP-biogenic)", "lang": "de"}], "type": "LCIA method data set", "refObjectId": "a7ea186c-9749-11ed-a8fc-0242ac120002", "version": "24.01.000", "uri": "../lciamethods/a7ea186c-9749-11ed-a8fc-0242ac120002.xml"}, "other": {"anies": [{"value": "0.00411271491493937", "module": "B6"}, {"name": "referenceToUnitGroupDataSet", "value": {"shortDescription": [{"value": "kg CO2 eq.", "lang": "en"}], "type": "unit group data set", "refObjectId": "1ebf3012-d0db-4de2-aefd-ef30cedb0be1", "version": "25.00.000", "uri": "../unitgroups/1ebf3012-d0db-4de2-aefd-ef30cedb0be1.xml"}}]}}, {"referenceToLCIAMethodDataSet": {"shortDescription": [{"value": "Climate change-Land use and land use change", "lang": "en"}, {"value": "Globales Erwärmungspotenzial - luluc (GWP-luluc)", "lang": "de"}], "type": "LCIA method data set", "refObjectId": "a7ea1ae2-9749-11ed-a8fc-0242ac120002", "version": "24.01.000", "uri": "../lciamethods/a7ea1ae2-9749-11ed-a8fc-0242ac120002.xml"}, "other": {"anies": [{"value": "6.84375690958505E-5", "module": "B6"}, {"name": "referenceToUnitGroupDataSet", "value": {"shortDescription": [{"value": "kg CO2 eq.", "lang": "en"}], "type": "unit group data set", "refObjectId": "1ebf3012-d0db-4de2-aefd-ef30cedb0be1", "version": "25.00.000", "uri": "../unitgroups/1ebf3012-d0db-4de2-aefd-ef30cedb0be1.xml"}}]}}, {"referenceToLCIAMethodDataSet": {"shortDescription": [{"value": "Depletion potenzial of the stratospheric ozone layer (ODP)", "lang": "en"}, {"value": "Abbaupotenzial der stratosphärischen Ozonschicht (ODP)", "lang": "de"}], "type": "LCIA method data set", "refObjectId": "b5c629d6-def3-11e6-bf01-fe55135034f3", "version": "24.01.000", "uri": "../lciamethods/b5c629d6-def3-11e6-bf01-fe55135034f3.xml"}, "other": {"anies": [{"value": "2.22941868764531E-11", "module": "B6"}, {"name": "referenceToUnitGroupDataSet", "value": {"shortDescription": [{"value": "kg CFC-11 eq.", "lang": "en"}], "type": "unit group data set", "refObjectId": "d9e957c9-7309-4474-bf3a-7777df6c4e5b", "version": "25.00.000", "uri": "../unitgroups/d9e957c9-7309-4474-bf3a-7777df6c4e5b.xml"}}]}}, {"referenceToLCIAMethodDataSet": {"shortDescription": [{"value": "Acidifcation potential, Accumulated Exceedance (AP)", "lang": "en"}, {"value": "Versauerungspotenzial, kumulierte Überschreitung (AP)", "lang": "de"}], "type": "LCIA method data set", "refObjectId": "b5c611c6-def3-11e6-bf01-fe55135034f3", "version": "24.01.000", "uri": "../lciamethods/b5c611c6-def3-11e6-bf01-fe55135034f3.xml"}, "other": {"anies": [{"value": "0.000537080240531012", "module": "B6"}, {"name": "referenceToUnitGroupDataSet", "value": {"shortDescription": [{"value": "Mole of H+ eq.", "lang": "en"}], "type": "unit group data set", "refObjectId": "42e089ac-92bf-4bf2-8ca1-5fc40d18f2ed", "version": "00.01.000", "uri": "../unitgroups/42e089ac-92bf-4bf2-8ca1-5fc40d18f2ed.xml"}}]}}, {"referenceToLCIAMethodDataSet": {"shortDescription": [{"value": "Eutrophication, freshwater", "lang": "en"}, {"value": "Eutrophierungspotenzial - Süßwasser (EP-freshwater)", "lang": "de"}], "type": "LCIA method data set", "refObjectId": "b53ec18f-7377-4ad3-86eb-cc3f4f276b2b", "version": "24.01.000", "uri": "../lciamethods/b53ec18f-7377-4ad3-86eb-cc3f4f276b2b.xml"}, "other": {"anies": [{"value": "1.83056384799292E-6", "module": "B6"}, {"name": "referenceToUnitGroupDataSet", "value": {"shortDescription": [{"value": "kg P eq.", "lang": "en"}], "type": "unit group data set", "refObjectId": "0429039d-a61d-4590-ba67-aa4a20a810a1", "version": "25.00.000", "uri": "../unitgroups/0429039d-a61d-4590-ba67-aa4a20a810a1.xml"}}]}}, {"referenceToLCIAMethodDataSet": {"shortDescription": [{"value": "Eutrophication marine", "lang": "en"}, {"value": "Eutrophierungspotenzial - Salzwasser (EP-marine)", "lang": "de"}], "type": "LCIA method data set", "refObjectId": "b5c619fa-def3-11e6-bf01-fe55135034f3", "version": "24.01.000", "uri": "../lciamethods/b5c619fa-def3-11e6-bf01-fe55135034f3.xml"}, "other": {"anies": [{"value": "0.000164151146145184", "module": "B6"}, {"name": "referenceToUnitGroupDataSet", "value": {"shortDescription": [{"value": "kg N eq.", "lang": "en"}], "type": "unit group data set", "refObjectId": "d05bb823-ecdf-4686-8c40-bf1d9257859f", "version": "00.00.003", "uri": "../unitgroups/d05bb823-ecdf-4686-8c40-bf1d9257859f.xml"}}]}}, {"referenceToLCIAMethodDataSet": {"shortDescription": [{"value": "Eutrophication, terrestrial", "lang": "en"}, {"value": "Eutrophierungspotenzial - Land (EP-terrestrial)", "lang": "de"}], "type": "LCIA method data set", "refObjectId": "b5c614d2-def3-11e6-bf01-fe55135034f3", "version": "24.01.000", "uri": "../lciamethods/b5c614d2-def3-11e6-bf01-fe55135034f3.xml"}, "other": {"anies": [{"value": "0.00171287446795714", "module": "B6"}, {"name": "referenceToUnitGroupDataSet", "value": {"shortDescription": [{"value": "Mole of N eq.", "lang": "en"}], "type": "unit group data set", "refObjectId": "71b4d617-0ec9-4d3f-b65e-e438940c2401", "version": "00.00.003", "uri": "../unitgroups/71b4d617-0ec9-4d3f-b65e-e438940c2401.xml"}}]}}, {"referenceToLCIAMethodDataSet": {"shortDescription": [{"value": "Photochemical Ozone Creation Potential  (POCP)", "lang": "en"}, {"value": "Bildungspotenzial für troposphärisches Ozon (POCP)", "lang": "de"}], "type": "LCIA method data set", "refObjectId": "b5c610fe-def3-11e6-bf01-fe55135034f3", "version": "24.01.000", "uri": "../lciamethods/b5c610fe-def3-11e6-bf01-fe55135034f3.xml"}, "other": {"anies": [{"value": "0.000404257488929039", "module": "B6"}, {"name": "referenceToUnitGroupDataSet", "value": {"shortDescription": [{"value": "kg NMVOC eq.", "lang": "en"}], "type": "unit group data set", "refObjectId": "d27c25f8-fbc1-44c6-b47b-4adbae4199c6", "version": "00.00.003", "uri": "../unitgroups/d27c25f8-fbc1-44c6-b47b-4adbae4199c6.xml"}}]}}, {"referenceToLCIAMethodDataSet": {"shortDescription": [{"value": "Resource use, minerals and metals", "lang": "en"}, {"value": "Potenzial für die Verknappung abiotischer Ressourcen  nicht fossile Ressourcen (ADPE)", "lang": "de"}], "type": "LCIA method data set", "refObjectId": "b2ad6494-c78d-11e6-9d9d-cec0c932ce01", "version": "24.01.000", "uri": "../lciamethods/b2ad6494-c78d-11e6-9d9d-cec0c932ce01.xml"}, "other": {"anies": [{"value": "1.01483532697023E-7", "module": "B6"}, {"name": "referenceToUnitGroupDataSet", "value": {"shortDescription": [{"value": "kg Sb eq.", "lang": "en"}], "type": "unit group data set", "refObjectId": "54ccd2d9-a32a-4fc2-923d-f2c8c93e89d4", "version": "25.00.000", "uri": "../unitgroups/54ccd2d9-a32a-4fc2-923d-f2c8c93e89d4.xml"}}]}}, {"referenceToLCIAMethodDataSet": {"shortDescription": [{"value": "Resource use, fossils", "lang": "en"}, {"value": "Potenzial für die Verknappung abiotischer Ressourcen  fossile Brennstoffe (ADPF)", "lang": "de"}], "type": "LCIA method data set", "refObjectId": "b2ad6110-c78d-11e6-9d9d-cec0c932ce01", "version": "24.01.000", "uri": "../lciamethods/b2ad6110-c78d-11e6-9d9d-cec0c932ce01.xml"}, "other": {"anies": [{"value": "3.76311674178447", "module": "B6"}, {"name": "referenceToUnitGroupDataSet", "value": {"shortDescription": [{"value": "MJ", "lang": "en"}], "type": "unit group data set", "refObjectId": "93a60a57-a3c8-11da-a746-0800200c9a66", "version": "02.00.000", "uri": "../unitgroups/93a60a57-a3c8-11da-a746-0800200c9a66.xml"}}]}}, {"referenceToLCIAMethodDataSet": {"shortDescription": [{"value": "Water use", "lang": "en"}, {"value": "Wasser-Entzugspotenzial (Benutzer) (WDP)", "lang": "de"}], "type": "LCIA method data set", "refObjectId": "b2ad66ce-c78d-11e6-9d9d-cec0c932ce01", "version": "24.01.000", "uri": "../lciamethods/b2ad66ce-c78d-11e6-9d9d-cec0c932ce01.xml"}, "other": {"anies": [{"value": "0.0121752995688224", "module": "B6"}, {"name": "referenceToUnitGroupDataSet", "value": {"shortDescription": [{"value": "m³ world equiv.", "lang": "en"}], "type": "unit group data set", "refObjectId": "6ae2df01-888e-46c8-b17d-49fa3869b476", "version": "00.00.003", "uri": "../unitgroups/6ae2df01-888e-46c8-b17d-49fa3869b476.xml"}}]}}]}, "otherAttributes": {"{http://www.indata.network/EPD/2019}epd-version": "1.2"}, "version": "1.1", "locations": "../ILCDLocations.xml"}