{"processInformation": {"dataSetInformation": {"UUID": "1e945704-b079-4b7f-b826-a6e44bba8a22", "name": {"baseName": [{"value": "ALPOLIC™  Composites (Mitsubishi Polyester Film GmbH)", "lang": "en"}, {"value": "ALPOLIC™ Verbundwerkstoffe (Mitsubishi Polyester Film GmbH)", "lang": "de"}]}, "classificationInformation": {"classification": [{"class": [{"value": "Metalle", "level": 0, "classId": "4"}, {"value": "Aluminium", "level": 1, "classId": "4.3"}, {"value": "Aluminiumbleche", "level": 2, "classId": "4.3.01"}], "name": "OEKOBAU.DAT"}]}, "generalComment": [{"value": "ALPOLIC Verbundwerkstoffe werden durch die Mitsubishi Polyester Film GmbH – Alpolic Division, sesshaft in Wiesbaden gefertigt. Betrachtet wurde ein durchschnittliches Produkt aus der Produktreihe ALPOLIC R85™ A1 und A2 ACM, ALPOLIC R85™ fr ACM und ALPOLIC R85™ real anodised. Die Umweltauswirkungen wurden für das Produkt mit der durchschnittlichen Rohdichte ausgewiesen. Der Deklarationsinhaber haftet für die zugrundeliegenden Angaben und Nachweise. Eine Haftung der Kiwa-Ecobility Experts (Kiwa GmbH) in Bezug auf Herstellerinformationen, Ökobilanzdaten und Nachweise ist ausgeschlossen.", "lang": "de"}, {"value": "ALPOLIC aluminium composite panels are manufactured by Mitsubishi Polyester Film GmbH - Alpolic Division, based in Wiesbaden. An average product from the range ALPOLIC R85™ A1 und A2 ACM, ALPOLIC R85™ fr ACM und ALPOLIC R85™ real anodized was considered. The environmental impacts were shown for the product with the average raw density. The declaration owner is liable for the underlying information and evidence, any liability of Kiwa-Ecobility Experts with regard to manufacturer information, LCA data and evidence is excluded.", "lang": "en"}], "other": {"anies": [{}, {"scenario": [{"description": [{"value": "In the case of PE-based adhesive and protective films, rubber and resin components are partly specified in the product data sheets. For simplification and due to the low overall relevance to the result, it ", "lang": "en"}], "name": "Standard scenario", "default": true}]}, "<ns11:modules xmlns:ns11=\"http://openlca.org/epd_ilcd\" xmlns=\"http://lca.jrc.it/ILCD/Process\" xmlns:c=\"http://lca.jrc.it/ILCD/Contact\" xmlns:common=\"http://lca.jrc.it/ILCD/Common\" xmlns:epd=\"http://www.iai.kit.edu/EPD/2013\" xmlns:epd2=\"http://www.indata.network/EPD/2019\" xmlns:f=\"http://lca.jrc.it/ILCD/Flow\" xmlns:fp=\"http://lca.jrc.it/ILCD/FlowProperty\" xmlns:m=\"http://lca.jrc.it/ILCD/LCIAMethod\" xmlns:ns9=\"http://www.okworx.com/ILCD/Extensions/2018/Profile\" xmlns:s=\"http://lca.jrc.it/ILCD/Source\" xmlns:u=\"http://lca.jrc.it/ILCD/UnitGroup\" name=\"A1\" scenario=\"Standard scenario\"/>", "<ns11:modules xmlns:ns11=\"http://openlca.org/epd_ilcd\" xmlns=\"http://lca.jrc.it/ILCD/Process\" xmlns:c=\"http://lca.jrc.it/ILCD/Contact\" xmlns:common=\"http://lca.jrc.it/ILCD/Common\" xmlns:epd=\"http://www.iai.kit.edu/EPD/2013\" xmlns:epd2=\"http://www.indata.network/EPD/2019\" xmlns:f=\"http://lca.jrc.it/ILCD/Flow\" xmlns:fp=\"http://lca.jrc.it/ILCD/FlowProperty\" xmlns:m=\"http://lca.jrc.it/ILCD/LCIAMethod\" xmlns:ns9=\"http://www.okworx.com/ILCD/Extensions/2018/Profile\" xmlns:s=\"http://lca.jrc.it/ILCD/Source\" xmlns:u=\"http://lca.jrc.it/ILCD/UnitGroup\" name=\"A2\" scenario=\"Standard scenario\"/>", "<ns11:modules xmlns:ns11=\"http://openlca.org/epd_ilcd\" xmlns=\"http://lca.jrc.it/ILCD/Process\" xmlns:c=\"http://lca.jrc.it/ILCD/Contact\" xmlns:common=\"http://lca.jrc.it/ILCD/Common\" xmlns:epd=\"http://www.iai.kit.edu/EPD/2013\" xmlns:epd2=\"http://www.indata.network/EPD/2019\" xmlns:f=\"http://lca.jrc.it/ILCD/Flow\" xmlns:fp=\"http://lca.jrc.it/ILCD/FlowProperty\" xmlns:m=\"http://lca.jrc.it/ILCD/LCIAMethod\" xmlns:ns9=\"http://www.okworx.com/ILCD/Extensions/2018/Profile\" xmlns:s=\"http://lca.jrc.it/ILCD/Source\" xmlns:u=\"http://lca.jrc.it/ILCD/UnitGroup\" name=\"A3\" scenario=\"Standard scenario\"/>", "<ns11:modules xmlns:ns11=\"http://openlca.org/epd_ilcd\" xmlns=\"http://lca.jrc.it/ILCD/Process\" xmlns:c=\"http://lca.jrc.it/ILCD/Contact\" xmlns:common=\"http://lca.jrc.it/ILCD/Common\" xmlns:epd=\"http://www.iai.kit.edu/EPD/2013\" xmlns:epd2=\"http://www.indata.network/EPD/2019\" xmlns:f=\"http://lca.jrc.it/ILCD/Flow\" xmlns:fp=\"http://lca.jrc.it/ILCD/FlowProperty\" xmlns:m=\"http://lca.jrc.it/ILCD/LCIAMethod\" xmlns:ns9=\"http://www.okworx.com/ILCD/Extensions/2018/Profile\" xmlns:s=\"http://lca.jrc.it/ILCD/Source\" xmlns:u=\"http://lca.jrc.it/ILCD/UnitGroup\" name=\"C1\" scenario=\"Standard scenario\"/>", "<ns11:modules xmlns:ns11=\"http://openlca.org/epd_ilcd\" xmlns=\"http://lca.jrc.it/ILCD/Process\" xmlns:c=\"http://lca.jrc.it/ILCD/Contact\" xmlns:common=\"http://lca.jrc.it/ILCD/Common\" xmlns:epd=\"http://www.iai.kit.edu/EPD/2013\" xmlns:epd2=\"http://www.indata.network/EPD/2019\" xmlns:f=\"http://lca.jrc.it/ILCD/Flow\" xmlns:fp=\"http://lca.jrc.it/ILCD/FlowProperty\" xmlns:m=\"http://lca.jrc.it/ILCD/LCIAMethod\" xmlns:ns9=\"http://www.okworx.com/ILCD/Extensions/2018/Profile\" xmlns:s=\"http://lca.jrc.it/ILCD/Source\" xmlns:u=\"http://lca.jrc.it/ILCD/UnitGroup\" name=\"C2\" scenario=\"Standard scenario\"/>", "<ns11:modules xmlns:ns11=\"http://openlca.org/epd_ilcd\" xmlns=\"http://lca.jrc.it/ILCD/Process\" xmlns:c=\"http://lca.jrc.it/ILCD/Contact\" xmlns:common=\"http://lca.jrc.it/ILCD/Common\" xmlns:epd=\"http://www.iai.kit.edu/EPD/2013\" xmlns:epd2=\"http://www.indata.network/EPD/2019\" xmlns:f=\"http://lca.jrc.it/ILCD/Flow\" xmlns:fp=\"http://lca.jrc.it/ILCD/FlowProperty\" xmlns:m=\"http://lca.jrc.it/ILCD/LCIAMethod\" xmlns:ns9=\"http://www.okworx.com/ILCD/Extensions/2018/Profile\" xmlns:s=\"http://lca.jrc.it/ILCD/Source\" xmlns:u=\"http://lca.jrc.it/ILCD/UnitGroup\" name=\"C3\" scenario=\"Standard scenario\"/>", "<ns11:modules xmlns:ns11=\"http://openlca.org/epd_ilcd\" xmlns=\"http://lca.jrc.it/ILCD/Process\" xmlns:c=\"http://lca.jrc.it/ILCD/Contact\" xmlns:common=\"http://lca.jrc.it/ILCD/Common\" xmlns:epd=\"http://www.iai.kit.edu/EPD/2013\" xmlns:epd2=\"http://www.indata.network/EPD/2019\" xmlns:f=\"http://lca.jrc.it/ILCD/Flow\" xmlns:fp=\"http://lca.jrc.it/ILCD/FlowProperty\" xmlns:m=\"http://lca.jrc.it/ILCD/LCIAMethod\" xmlns:ns9=\"http://www.okworx.com/ILCD/Extensions/2018/Profile\" xmlns:s=\"http://lca.jrc.it/ILCD/Source\" xmlns:u=\"http://lca.jrc.it/ILCD/UnitGroup\" name=\"C4\" scenario=\"Standard scenario\"/>", "<ns11:modules xmlns:ns11=\"http://openlca.org/epd_ilcd\" xmlns=\"http://lca.jrc.it/ILCD/Process\" xmlns:c=\"http://lca.jrc.it/ILCD/Contact\" xmlns:common=\"http://lca.jrc.it/ILCD/Common\" xmlns:epd=\"http://www.iai.kit.edu/EPD/2013\" xmlns:epd2=\"http://www.indata.network/EPD/2019\" xmlns:f=\"http://lca.jrc.it/ILCD/Flow\" xmlns:fp=\"http://lca.jrc.it/ILCD/FlowProperty\" xmlns:m=\"http://lca.jrc.it/ILCD/LCIAMethod\" xmlns:ns9=\"http://www.okworx.com/ILCD/Extensions/2018/Profile\" xmlns:s=\"http://lca.jrc.it/ILCD/Source\" xmlns:u=\"http://lca.jrc.it/ILCD/UnitGroup\" name=\"D\" scenario=\"Standard scenario\"/>", {}]}}, "quantitativeReference": {"referenceToReferenceFlow": [1], "type": "Reference flow(s)"}, "time": {"referenceYear": 2023, "dataSetValidUntil": 2030, "timeRepresentativenessDescription": [{"value": "Die Produktionsdaten wurden im Betriebsjahr 2021 (01.01.2021-31.12.2021) erhoben und im Jahr 2023 aktualisiert (01.01.2023-31.12.2023)", "lang": "de"}, {"value": "The production data was collected in the operating year 2021 (01.01.2021-31.12.2021) and updated in 2023 (01.01.2023-31.12.2023). ", "lang": "en"}], "other": {"anies": [{"name": "publicationDateOfEPD", "value": 1744243200000}]}}, "geography": {"locationOfOperationSupplyOrProduction": {"descriptionOfRestrictions": [{"value": "The geographical reference area is Germany (Wiesbaden).\r", "lang": "en"}, {"value": "Als geographischer Referenzraum dient Deutschland (Wiesbaden).", "lang": "de"}], "location": "DE"}}, "technology": {"technologyDescriptionAndIncludedProcesses": [{"value": "ALPOLIC™ Verbundwerkstoffe sind dünne Platten bestehend aus zwei dünnen Aluminiumplatten (in diesem Fall mindestens 85 Gew. % rezykliertes Aluminium) auf beiden Seiten und einem thermoplastischen oder mineralgefüllten, feuerhemmenden Kern. Die bereits lackierten Aluminiumoberflächen werden mit einer Klebefolie versehen und im Anschluss mit dem Kernmaterial laminiert. ALPOLIC™ -Produkte bieten eine große Auswahl an Oberflächenarten, Farben und Glanzgraden für Gebäude. Sie werden mit robustem und stabilem Fluorpolymerlack beschichtet, damit die Oberflächen auch nach jahrzehntelanger Einwirkung von Wettereinflüssen frisch bleiben. Dabei bieten die ALPOLIC™ Verbundwerkstoffe die Steifigkeit von schwerem Blech in einem leichten Verbundwerkstoff.\r\n\r\nALPOLIC™ Aluminium-Verbundwerkstoffe (ACM) werden in Wiesbaden, Deutschland hergestellt. Das Produkt wird durch kontinuierliches Verbinden von zwei Aluminiumcoils auf beiden Seiten eines extrudierten thermoplastischen oder mineralgefüllten, feuerhemmenden thermoplastischen Kerns hergestellt. Die Aluminiumoberflächen wurden vorveredelt und vor dem Verkleben in verschiedenen Lackierungen bandbeschichtet (Extrusion des thermoplastischen Kerns, Laminierung mit den Aluminiumcoils, Transporte innerhalb des Werks, A3).\r\n", "lang": "de"}, {"value": "ALPOLIC™ Composites are thin panels consisting of two thin aluminium plates (in this case at least 85 % by weight of recycled aluminum) on both sides and a thermoplastic or mineral-filled, fire-retardant core. The already painted aluminium surfaces are provided with an adhesive film and subsequently laminated with the core material. ALPOLIC ™ products offer a huge range of surface types, colours and gloss levels for buildings. They are coated with robust and stable fluoropolymer paint to keep surfaces fresh after decades of exposure to the elements. At the same time, ALPOLIC ™ composite panels offer the rigidity of heavy sheet metal in a lightweight composite material.\r\n\r\nALPOLIC™ Aluminium Composites (ACM) are manufactured in Wiesbaden, Germany. The product is manufactured by continuously bonding two aluminium coils on either side of an extruded thermoplastic or mineral-filled fire-retardant thermoplastic core. The aluminium surfaces have been pre-finished and coil-coated in various paint finishes before bonding (Extrusion of the thermoplastic core, lamination with the aluminum coils, transport within the plant, A3).\r\n", "lang": "en"}], "technologicalApplicability": [{"value": "ALPOLIC™-Verbundwerkstoffe sind für Architekturprojekte, sie können zu komplexen Formen verarbeitet werden und sind einfach zu installieren. Gleichzeitig bieten sie eine gute Planheit, Langlebigkeit, Stabilität, Vibrationsdämpfung und Wartungsfreundlichkeit. Damit eignen sie sich als Vorhangfassaden, Regenschutzsysteme und für andere Anwendungen von Architekturverkleidungen. ALPOLIC™ kann mit handelsüblichen Holz- oder Metallbearbeitungswerkzeugen ohne Spezialwerkzeug bearbeitet werden. Schneiden, Nuten, Stanzen, Bohren, Biegen, Walzen und viele andere Fertigungstechniken können durchgeführt werden, um komplexen Formen zu erzeugen.", "lang": "de"}, {"value": "ALPOLIC™ composite panels are ideal for architectural projects, they can be easily processed into complex shapes and are easy to install. At the same time, they offer excellent flatness, durability, stability, vibration damping and ease of maintenance. This makes them suitable for curtain walls, rainscreen systems and other architectural cladding applications. ALPOLIC™ can be machined with standard woodworking or metalworking tools without the need for special tools. Cutting, grooving, punching, drilling, bending, rolling and many other manufacturing techniques can be easily performed to create an almost unlimited variety of complex shapes and forms.", "lang": "en"}], "referenceToTechnologyFlowDiagrammOrPicture": [{"shortDescription": [{"value": "Flow chart ALPOLIC™ Composites", "lang": "en"}], "type": "source data set", "refObjectId": "58640b48-9e00-4a92-bb14-155461b0b6ae", "version": "00.00.003"}]}}, "modellingAndValidation": {"LCIMethodAndAllocation": {"typeOfDataSet": "EPD", "other": {"anies": [{"name": "subType", "value": "average dataset"}]}}, "dataSourcesTreatmentAndRepresentativeness": {"referenceToDataSource": [{"shortDescription": [{"value": "ecoinvent 3.8 database", "lang": "en"}], "type": "source data set", "refObjectId": "0f4c65c0-6210-450f-b886-82bf8dd5ace9", "version": "00.00.001"}, {"shortDescription": [{"value": "ecoinvent database (general)", "lang": "en"}], "type": "source data set", "refObjectId": "b497a91f-e14b-4b69-8f28-f50eb1576766", "version": "00.03.002"}, {"shortDescription": [{"value": "GaBi database (general)", "lang": "en"}], "type": "source data set", "refObjectId": "28d74cc0-db8b-4d7e-bc44-5f6d56ce0c4a", "version": "00.03.002"}, {"shortDescription": [{"value": "Sphera MLC (fka GaBi) Databases Edition 2024", "lang": "en"}], "type": "source data set", "refObjectId": "7443b962-0446-4d69-8aa7-8055a6b1614a", "version": "00.01.000"}], "useAdviceForDataSet": [{"value": "ALPOLIC™-Verbundwerkstoffe sind für Architekturprojekte, sie können zu komplexen Formen verarbeitet werden und sind einfach zu installieren. Gleichzeitig bieten sie eine gute Planheit, Langlebigkeit, Stabilität, Vibrationsdämpfung und Wartungsfreundlichkeit. Damit eignen sie sich als Vorhangfassaden, Regenschutzsysteme und für andere Anwendungen von Architekturverkleidungen. ALPOLIC™ kann mit handelsüblichen Holz- oder Metallbearbeitungswerkzeugen ohne Spezialwerkzeug bearbeitet werden. Schneiden, Nuten, Stanzen, Bohren, Biegen, Walzen und viele andere Fertigungstechniken können durchgeführt werden, um komplexen Formen zu erzeugen.", "lang": "de"}, {"value": "ALPOLIC™ composite panels are ideal for architectural projects, they can be easily processed into complex shapes and are easy to install. At the same time, they offer excellent flatness, durability, stability, vibration damping and ease of maintenance. This makes them suitable for curtain walls, rainscreen systems and other architectural cladding applications. ALPOLIC™ can be machined with standard woodworking or metalworking tools without the need for special tools. Cutting, grooving, punching, drilling, bending, rolling and many other manufacturing techniques can be easily performed to create an almost unlimited variety of complex shapes and forms.", "lang": "en"}], "other": {"anies": [{"name": "referenceToOriginalEPD", "value": {"shortDescription": {"value": "ALPOLIC™ Composites EPD ", "defaultValue": "ALPOLIC™ Composites EPD ", "lstrings": [{"lang": "en", "value": "ALPOLIC™ Composites EPD "}]}, "version": {"version": 6, "majorVersion": 0, "minorVersion": 0, "subMinorVersion": 6, "zero": false, "versionString": "00.00.006"}, "type": "source data set", "uuid": {"uuid": "eec5d031-ff71-49ab-ae9e-0a6803c94d36"}, "refObjectId": "eec5d031-ff71-49ab-ae9e-0a6803c94d36", "versionAsString": "00.00.006", "resourceURLs": ["https://oekobaudat.de/OEKOBAU.DAT/resource/sources/eec5d031-ff71-49ab-ae9e-0a6803c94d36/EPD-Kiwa-EE-000424-DE.pdf?version=00.00.006", "https://oekobaudat.de/OEKOBAU.DAT/resource/sources/eec5d031-ff71-49ab-ae9e-0a6803c94d36/EPD-Kiwa-EE-000425-EN.pdf?version=00.00.006"]}}]}}, "validation": {"review": [{"reviewDetails": [{"value": "Unabhängige Verifizierung der EPD durch eine/n unabhängige/n Dritte/n gemäß ISO 14025:2011-10.", "lang": "de"}, {"value": "Independent verification of the declaration and data according to ISO 14025:2011-10\r.", "lang": "en"}], "referenceToNameOfReviewerAndInstitution": [{"shortDescription": [{"value": "Martin Köhrer (External verifier of Kiwa GmbH)", "lang": "en"}], "type": "contact data set", "refObjectId": "1e034da6-8bef-4bf8-8695-b29bc04623ab", "version": "00.00.001"}], "type": "Independent external review"}]}, "complianceDeclarations": {"compliance": [{"referenceToComplianceSystem": {"shortDescription": [{"value": "ISO 14025", "lang": "en"}], "type": "source data set", "refObjectId": "4f2eb655-6e44-4874-a95a-e28f5442cd4d", "version": "00.00.001"}}, {"referenceToComplianceSystem": {"shortDescription": [{"value": "EN 15804+A2 (EF 3.1)", "lang": "de"}, {"value": "EN 15804+A2 (EF 3.1)", "lang": "en"}], "type": "source data set", "refObjectId": "d4aa3ec7-b1d7-4a4a-a6cb-37af88dcc902", "version": "00.01.000"}}]}}, "administrativeInformation": {"commissionerAndGoal": {"referenceToCommissioner": [{"shortDescription": [{"value": "Mitsubishi Polyester Film GmbH", "lang": "en"}], "type": "contact data set", "refObjectId": "1603df25-7263-4afe-8daa-a58032d704fd", "version": "00.00.002"}]}, "dataGenerator": {"referenceToPersonOrEntityGeneratingTheDataSet": [{"shortDescription": [{"value": "Mitsubishi Chemical Europe GmbH, Dr Bálint Simon", "lang": "en"}], "type": "contact data set", "refObjectId": "192b726a-5e71-47fe-a9e6-c12247c346c2", "version": "00.00.001"}]}, "dataEntryBy": {"timeStamp": 1746538189243, "referenceToDataSetFormat": [{"shortDescription": [{"value": "EPD Data Format Extensions v1.2", "lang": "en"}, {"value": "EPD-Datenformaterweiterungen v1.2", "lang": "de"}], "type": "source data set", "refObjectId": "a29449fd-aa2f-4de8-b5d7-4b06b43c6fde", "version": "00.01.000"}, {"shortDescription": [{"value": "ILCD format", "lang": "en"}], "type": "source data set", "refObjectId": "a97a0155-0234-4b87-b4ce-a45da52f2a40", "version": "01.00.001", "uri": "http://lca.jrc.ec.europa.eu/lcainfohub/sample_data/ilcd/sources/ILCD_Format_a97a0155-0234-4b87-b4ce-a45da52f2a40_01.00.000.xml"}], "referenceToPersonOrEntityEnteringTheData": {"shortDescription": [{"value": "Kiwa-Ecobility Experts, Kiwa GmbH (Berlin)", "lang": "en"}], "type": "contact data set", "refObjectId": "eb52a9a8-9d0f-40ce-a5c9-7b78f5615e5a", "version": "00.00.002"}}, "publicationAndOwnership": {"dataSetVersion": "00.00.062", "referenceToRegistrationAuthority": {"shortDescription": [{"value": "Kiwa-Ecobility Experts, Kiwa GmbH (Berlin)", "lang": "en"}], "type": "contact data set", "refObjectId": "eb52a9a8-9d0f-40ce-a5c9-7b78f5615e5a", "version": "00.00.002"}, "registrationNumber": "EPD-Kiwa-EE-000425-EN; EPD-Kiwa-EE-000424-DE", "referenceToOwnershipOfDataSet": {"shortDescription": [{"value": "Mitsubishi Polyester Film GmbH", "lang": "en"}], "type": "contact data set", "refObjectId": "1603df25-7263-4afe-8daa-a58032d704fd", "version": "00.00.002"}, "copyright": true, "licenseType": "Free of charge for all users and uses", "accessRestrictions": [{"value": "Keine.", "lang": "de"}, {"value": "None.", "lang": "en"}], "other": {"anies": [{"name": "referenceToPublisher", "value": {"shortDescription": [{"value": "Kiwa-Ecobility Experts, Kiwa GmbH (Berlin)", "lang": "en"}], "type": "contact data set", "refObjectId": "eb52a9a8-9d0f-40ce-a5c9-7b78f5615e5a", "version": "00.00.002"}}]}}}, "exchanges": {"exchange": [{"dataSetInternalID": 1, "referenceToFlowDataSet": {"shortDescription": [{"value": "ALPOLIC™ Verbundwerkstoffe", "lang": "de"}, {"value": "ALPOLIC™ Composites", "lang": "en"}], "type": "flow data set", "refObjectId": "069e4829-53d4-491f-902e-2121b9705958", "version": "00.00.013"}, "meanAmount": 1.0, "resultingAmount": 1.0, "referenceFlow": true, "resultingflowAmount": 1.0, "flowProperties": [{"name": [{"lang": "de", "value": "Fläche"}, {"lang": "en", "value": "Area"}], "uuid": "93a60a56-a3c8-19da-a746-0800200c9a66", "referenceFlowProperty": true, "meanValue": 1.0, "referenceUnit": "qm", "unitGroupUUID": "c20a03d7-bd90-4569-bc94-66cfd364dfc8"}], "materialProperties": [{"name": "grammage", "value": "7.76", "unit": "kg/m^2", "unitDescription": "kilograms per square meter"}, {"name": "layer thickness", "value": "0.004", "unit": "m", "unitDescription": "meters"}], "typeOfFlow": "Product flow", "classification": {"classHierarchy": "Metalle / Aluminium / Aluminiumbleche", "name": "OEKOBAU.DAT"}}, {"dataSetInternalID": 2, "referenceToFlowDataSet": {"shortDescription": [{"value": "Components for re-use (CRU)", "lang": "en"}, {"value": "Komponenten für die Wiederverwendung (CRU)", "lang": "de"}, {"value": "Componentes para su reutilización (CRU)", "lang": "es"}], "type": "flow data set", "refObjectId": "a2b32f97-3fc7-4af2-b209-525bc6426f33", "version": "30.00.000", "uri": "../flows/a2b32f97-3fc7-4af2-b209-525bc6426f33.xml"}, "exchange direction": "OUTPUT", "meanAmount": 0.0, "other": {"anies": [{"value": "0.0", "module": "A1", "scenario": "Standard scenario"}, {"value": "0.0", "module": "A2", "scenario": "Standard scenario"}, {"value": "0.0", "module": "A3", "scenario": "Standard scenario"}, {"value": "0.0", "module": "C1", "scenario": "Standard scenario"}, {"value": "0.0", "module": "C2", "scenario": "Standard scenario"}, {"value": "0.0", "module": "C3", "scenario": "Standard scenario"}, {"value": "0.0", "module": "C4", "scenario": "Standard scenario"}, {"value": "0.0", "module": "D", "scenario": "Standard scenario"}, {"name": "referenceToUnitGroupDataSet", "value": {"shortDescription": [{"value": "kg", "lang": "en"}], "type": "unit group data set", "refObjectId": "ad38d542-3fe9-439d-9b95-2f5f7752acaf", "version": "30.00.000", "uri": "../unitgroups/ad38d542-3fe9-439d-9b95-2f5f7752acaf.xml"}}]}, "flowProperties": [], "typeOfFlow": "Other flow", "classification": {"classHierarchy": "Größen / Umweltliche Größen / EPD EN 15804 / LCI Indikatoren", "name": "GaBiCategories"}}, {"dataSetInternalID": 3, "referenceToFlowDataSet": {"shortDescription": [{"value": "Exported electrical energy (EEE)", "lang": "en"}, {"value": "Exportierte elektrische Energie (EEE)", "lang": "de"}, {"value": "Energía exportada electrica (EEE)", "lang": "es"}], "type": "flow data set", "refObjectId": "4da0c987-2b76-40d6-9e9e-82a017aaaf29", "version": "30.00.000", "uri": "../flows/4da0c987-2b76-40d6-9e9e-82a017aaaf29.xml"}, "exchange direction": "OUTPUT", "meanAmount": 0.0, "other": {"anies": [{"value": "0.0", "module": "A1", "scenario": "Standard scenario"}, {"value": "0.0", "module": "A2", "scenario": "Standard scenario"}, {"value": "0.193", "module": "A3", "scenario": "Standard scenario"}, {"value": "0.0", "module": "C1", "scenario": "Standard scenario"}, {"value": "0.0", "module": "C2", "scenario": "Standard scenario"}, {"value": "4.48", "module": "C3", "scenario": "Standard scenario"}, {"value": "0.0", "module": "C4", "scenario": "Standard scenario"}, {"value": "0.0", "module": "D", "scenario": "Standard scenario"}, {"name": "referenceToUnitGroupDataSet", "value": {"shortDescription": [{"value": "MJ", "lang": "en"}], "type": "unit group data set", "refObjectId": "93a60a57-a3c8-11da-a746-0800200c9a66", "version": "03.00.000", "uri": "../unitgroups/93a60a57-a3c8-11da-a746-0800200c9a66.xml"}}]}, "flowProperties": [], "typeOfFlow": "Other flow", "classification": {"classHierarchy": "Größen / Umweltliche Größen / EPD EN 15804 / LCI Indikatoren", "name": "GaBiCategories"}}, {"dataSetInternalID": 4, "referenceToFlowDataSet": {"shortDescription": [{"value": "Exported thermal energy (EET)", "lang": "en"}, {"value": "Exportierte thermische Energie (EET)", "lang": "de"}, {"value": "Energía exportada termal (EET)", "lang": "es"}], "type": "flow data set", "refObjectId": "98daf38a-7a79-46d3-9a37-2b7bd0955810", "version": "30.00.000", "uri": "../flows/98daf38a-7a79-46d3-9a37-2b7bd0955810.xml"}, "exchange direction": "OUTPUT", "meanAmount": 0.0, "other": {"anies": [{"value": "0.0", "module": "A1", "scenario": "Standard scenario"}, {"value": "0.0", "module": "A2", "scenario": "Standard scenario"}, {"value": "0.444", "module": "A3", "scenario": "Standard scenario"}, {"value": "0.0", "module": "C1", "scenario": "Standard scenario"}, {"value": "0.0", "module": "C2", "scenario": "Standard scenario"}, {"value": "10.3", "module": "C3", "scenario": "Standard scenario"}, {"value": "0.0", "module": "C4", "scenario": "Standard scenario"}, {"value": "0.0", "module": "D", "scenario": "Standard scenario"}, {"name": "referenceToUnitGroupDataSet", "value": {"shortDescription": [{"value": "MJ", "lang": "en"}], "type": "unit group data set", "refObjectId": "93a60a57-a3c8-11da-a746-0800200c9a66", "version": "03.00.000", "uri": "../unitgroups/93a60a57-a3c8-11da-a746-0800200c9a66.xml"}}]}, "flowProperties": [], "typeOfFlow": "Other flow", "classification": {"classHierarchy": "Größen / Umweltliche Größen / EPD EN 15804 / LCI Indikatoren", "name": "GaBiCategories"}}, {"dataSetInternalID": 5, "referenceToFlowDataSet": {"shortDescription": [{"value": "Use of net fresh water (FW)", "lang": "en"}, {"value": "Einsatz von Süßwasserressourcen (FW)", "lang": "de"}, {"value": "Uso neto de recursos de agua dulce (FW)", "lang": "es"}], "type": "flow data set", "refObjectId": "3cf952c8-f3a4-461d-8c96-96456ca62246", "version": "30.00.000", "uri": "../flows/3cf952c8-f3a4-461d-8c96-96456ca62246.xml"}, "exchange direction": "INPUT", "meanAmount": 0.0, "other": {"anies": [{"value": "0.0716", "module": "A1", "scenario": "Standard scenario"}, {"value": "3.74E-4", "module": "A2", "scenario": "Standard scenario"}, {"value": "0.0242", "module": "A3", "scenario": "Standard scenario"}, {"value": "2.21E-4", "module": "C1", "scenario": "Standard scenario"}, {"value": "2.03E-5", "module": "C2", "scenario": "Standard scenario"}, {"value": "0.00665", "module": "C3", "scenario": "Standard scenario"}, {"value": "2.03E-4", "module": "C4", "scenario": "Standard scenario"}, {"value": "-0.0336", "module": "D", "scenario": "Standard scenario"}, {"name": "referenceToUnitGroupDataSet", "value": {"shortDescription": [{"value": "m3", "lang": "en"}], "type": "unit group data set", "refObjectId": "cd950537-0a98-4044-9ba7-9f9a68d0a504", "version": "30.00.000", "uri": "../unitgroups/cd950537-0a98-4044-9ba7-9f9a68d0a504.xml"}}]}, "flowProperties": [], "typeOfFlow": "Other flow", "classification": {"classHierarchy": "Größen / Umweltliche Größen / EPD EN 15804 / LCI Indikatoren", "name": "GaBiCategories"}}, {"dataSetInternalID": 6, "referenceToFlowDataSet": {"shortDescription": [{"value": "Hazardous waste disposed (HWD)", "lang": "en"}, {"value": "Gefährlicher Abfall zur Deponie (HWD)", "lang": "de"}, {"value": "Residuos peligrosos eliminados (HWD)", "lang": "es"}], "type": "flow data set", "refObjectId": "430f9e0f-59b2-46a0-8e0d-55e0e84948fc", "version": "30.00.000", "uri": "../flows/430f9e0f-59b2-46a0-8e0d-55e0e84948fc.xml"}, "exchange direction": "OUTPUT", "meanAmount": 0.0, "other": {"anies": [{"value": "6.2E-8", "module": "A1", "scenario": "Standard scenario"}, {"value": "2.0E-10", "module": "A2", "scenario": "Standard scenario"}, {"value": "3.09E-9", "module": "A3", "scenario": "Standard scenario"}, {"value": "9.11E-11", "module": "C1", "scenario": "Standard scenario"}, {"value": "6.91E-12", "module": "C2", "scenario": "Standard scenario"}, {"value": "2.17E-9", "module": "C3", "scenario": "Standard scenario"}, {"value": "1.92E-10", "module": "C4", "scenario": "Standard scenario"}, {"value": "-2.72E-8", "module": "D", "scenario": "Standard scenario"}, {"name": "referenceToUnitGroupDataSet", "value": {"shortDescription": [{"value": "kg", "lang": "en"}], "type": "unit group data set", "refObjectId": "ad38d542-3fe9-439d-9b95-2f5f7752acaf", "version": "30.00.000", "uri": "../unitgroups/ad38d542-3fe9-439d-9b95-2f5f7752acaf.xml"}}]}, "flowProperties": [], "typeOfFlow": "Other flow", "classification": {"classHierarchy": "Größen / Umweltliche Größen / EPD EN 15804 / LCI Indikatoren", "name": "GaBiCategories"}}, {"dataSetInternalID": 7, "referenceToFlowDataSet": {"shortDescription": [{"value": "Materials for energy recovery (MER)", "lang": "en"}, {"value": "Stoffe für die Energierückgewinnung (MER)", "lang": "de"}, {"value": "Materiales para valorización energética (recuperación de energía) (MER)", "lang": "es"}], "type": "flow data set", "refObjectId": "59a9181c-3aaf-46ee-8b13-2b3723b6e447", "version": "30.00.000", "uri": "../flows/59a9181c-3aaf-46ee-8b13-2b3723b6e447.xml"}, "exchange direction": "OUTPUT", "meanAmount": 0.0, "other": {"anies": [{"value": "0.0", "module": "A1", "scenario": "Standard scenario"}, {"value": "0.0", "module": "A2", "scenario": "Standard scenario"}, {"value": "0.0503", "module": "A3", "scenario": "Standard scenario"}, {"value": "0.0", "module": "C1", "scenario": "Standard scenario"}, {"value": "0.0", "module": "C2", "scenario": "Standard scenario"}, {"value": "1.17", "module": "C3", "scenario": "Standard scenario"}, {"value": "0.0", "module": "C4", "scenario": "Standard scenario"}, {"value": "0.0", "module": "D", "scenario": "Standard scenario"}, {"name": "referenceToUnitGroupDataSet", "value": {"shortDescription": [{"value": "kg", "lang": "en"}], "type": "unit group data set", "refObjectId": "ad38d542-3fe9-439d-9b95-2f5f7752acaf", "version": "30.00.000", "uri": "../unitgroups/ad38d542-3fe9-439d-9b95-2f5f7752acaf.xml"}}]}, "flowProperties": [], "typeOfFlow": "Other flow", "classification": {"classHierarchy": "Größen / Umweltliche Größen / EPD EN 15804 / LCI Indikatoren", "name": "GaBiCategories"}}, {"dataSetInternalID": 8, "referenceToFlowDataSet": {"shortDescription": [{"value": "Materials for recycling (MFR)", "lang": "en"}, {"value": "Stoffe zum Recycling (MFR)", "lang": "de"}, {"value": "Materiales para el reciclaje (MFR)", "lang": "es"}], "type": "flow data set", "refObjectId": "d7fe48a5-4103-49c8-9aae-b0b5dfdbd6ae", "version": "30.00.000", "uri": "../flows/d7fe48a5-4103-49c8-9aae-b0b5dfdbd6ae.xml"}, "exchange direction": "OUTPUT", "meanAmount": 0.0, "other": {"anies": [{"value": "0.0", "module": "A1", "scenario": "Standard scenario"}, {"value": "0.0", "module": "A2", "scenario": "Standard scenario"}, {"value": "0.261", "module": "A3", "scenario": "Standard scenario"}, {"value": "0.0", "module": "C1", "scenario": "Standard scenario"}, {"value": "0.0", "module": "C2", "scenario": "Standard scenario"}, {"value": "2.72", "module": "C3", "scenario": "Standard scenario"}, {"value": "0.0", "module": "C4", "scenario": "Standard scenario"}, {"value": "0.0", "module": "D", "scenario": "Standard scenario"}, {"name": "referenceToUnitGroupDataSet", "value": {"shortDescription": [{"value": "kg", "lang": "en"}], "type": "unit group data set", "refObjectId": "ad38d542-3fe9-439d-9b95-2f5f7752acaf", "version": "30.00.000", "uri": "../unitgroups/ad38d542-3fe9-439d-9b95-2f5f7752acaf.xml"}}]}, "flowProperties": [], "typeOfFlow": "Other flow", "classification": {"classHierarchy": "Größen / Umweltliche Größen / EPD EN 15804 / LCI Indikatoren", "name": "GaBiCategories"}}, {"dataSetInternalID": 9, "referenceToFlowDataSet": {"shortDescription": [{"value": "Non-hazardous waste disposed (NHWD)", "lang": "en"}, {"value": "Entsorgter nicht gefährlicher Abfall (NHWD)", "lang": "de"}, {"value": "Residuos no peligrosos eliminados (NHWD)", "lang": "es"}], "type": "flow data set", "refObjectId": "b29ef66b-e286-4afa-949f-62f1a7b4d7fa", "version": "30.00.000", "uri": "../flows/b29ef66b-e286-4afa-949f-62f1a7b4d7fa.xml"}, "exchange direction": "OUTPUT", "meanAmount": 0.0, "other": {"anies": [{"value": "5.69", "module": "A1", "scenario": "Standard scenario"}, {"value": "8.65E-4", "module": "A2", "scenario": "Standard scenario"}, {"value": "0.00336", "module": "A3", "scenario": "Standard scenario"}, {"value": "3.54E-4", "module": "C1", "scenario": "Standard scenario"}, {"value": "3.32E-5", "module": "C2", "scenario": "Standard scenario"}, {"value": "0.0578", "module": "C3", "scenario": "Standard scenario"}, {"value": "3.88", "module": "C4", "scenario": "Standard scenario"}, {"value": "-0.778", "module": "D", "scenario": "Standard scenario"}, {"name": "referenceToUnitGroupDataSet", "value": {"shortDescription": [{"value": "kg", "lang": "en"}], "type": "unit group data set", "refObjectId": "ad38d542-3fe9-439d-9b95-2f5f7752acaf", "version": "30.00.000", "uri": "../unitgroups/ad38d542-3fe9-439d-9b95-2f5f7752acaf.xml"}}]}, "flowProperties": [], "typeOfFlow": "Other flow", "classification": {"classHierarchy": "Größen / Umweltliche Größen / EPD EN 15804 / LCI Indikatoren", "name": "GaBiCategories"}}, {"dataSetInternalID": 10, "referenceToFlowDataSet": {"shortDescription": [{"value": "Use of non renewable secondary fuels (NRSF)", "lang": "en"}, {"value": "Nicht erneuerbare Sekundärbrennstoffe (NRSF)", "lang": "de"}, {"value": "Uso de combustibles secundarios no renovables (NRSF)", "lang": "es"}], "type": "flow data set", "refObjectId": "89def144-d39a-4287-b86f-efde453ddcb2", "version": "30.00.000", "uri": "../flows/89def144-d39a-4287-b86f-efde453ddcb2.xml"}, "exchange direction": "INPUT", "meanAmount": 0.0, "other": {"anies": [{"value": "0.0", "module": "A1", "scenario": "Standard scenario"}, {"value": "0.0", "module": "A2", "scenario": "Standard scenario"}, {"value": "0.0", "module": "A3", "scenario": "Standard scenario"}, {"value": "0.0", "module": "C1", "scenario": "Standard scenario"}, {"value": "0.0", "module": "C2", "scenario": "Standard scenario"}, {"value": "0.0", "module": "C3", "scenario": "Standard scenario"}, {"value": "0.0", "module": "C4", "scenario": "Standard scenario"}, {"value": "0.0", "module": "D", "scenario": "Standard scenario"}, {"name": "referenceToUnitGroupDataSet", "value": {"shortDescription": [{"value": "MJ", "lang": "en"}], "type": "unit group data set", "refObjectId": "93a60a57-a3c8-11da-a746-0800200c9a66", "version": "03.00.000", "uri": "../unitgroups/93a60a57-a3c8-11da-a746-0800200c9a66.xml"}}]}, "flowProperties": [], "typeOfFlow": "Other flow", "classification": {"classHierarchy": "Größen / Umweltliche Größen / EPD EN 15804 / LCI Indikatoren", "name": "GaBiCategories"}}, {"dataSetInternalID": 11, "referenceToFlowDataSet": {"shortDescription": [{"value": "Use of non renewable primary energy (PENRE)", "lang": "en"}, {"value": "Nicht-erneuerbare Primärenergie als Energieträger (PENRE)", "lang": "de"}, {"value": "Uso de energía primaria no renovable, excluyendo los recursos de energía primaria no renovable utilizada como materia prima (PENRE)", "lang": "es"}], "type": "flow data set", "refObjectId": "ac857178-2b45-46ec-892a-a9a4332f0372", "version": "38.00.000", "uri": "../flows/ac857178-2b45-46ec-892a-a9a4332f0372.xml"}, "exchange direction": "INPUT", "meanAmount": 0.0, "other": {"anies": [{"value": "208.0", "module": "A1", "scenario": "Standard scenario"}, {"value": "10.6", "module": "A2", "scenario": "Standard scenario"}, {"value": "7.06", "module": "A3", "scenario": "Standard scenario"}, {"value": "2.14", "module": "C1", "scenario": "Standard scenario"}, {"value": "0.214", "module": "C2", "scenario": "Standard scenario"}, {"value": "1.35", "module": "C3", "scenario": "Standard scenario"}, {"value": "0.766", "module": "C4", "scenario": "Standard scenario"}, {"value": "-55.8", "module": "D", "scenario": "Standard scenario"}, {"name": "referenceToUnitGroupDataSet", "value": {"shortDescription": [{"value": "MJ", "lang": "en"}], "type": "unit group data set", "refObjectId": "93a60a57-a3c8-11da-a746-0800200c9a66", "version": "03.00.000", "uri": "../unitgroups/93a60a57-a3c8-11da-a746-0800200c9a66.xml"}}]}, "flowProperties": [], "typeOfFlow": "Other flow", "classification": {"classHierarchy": "Quantities", "name": "GaBiCategories"}}, {"dataSetInternalID": 12, "referenceToFlowDataSet": {"shortDescription": [{"value": "Use of non renewable primary energy resources used as raw materials (PENRM)", "lang": "en"}, {"value": "Nicht-erneuerbare Primärenergie zur stofflichen Nutzung (PENRM)", "lang": "de"}, {"value": "Uso de la energía primaria no renovable utilizada como materia prima (PENRM)", "lang": "es"}], "type": "flow data set", "refObjectId": "1421caa0-679d-4bf4-b282-0eb850ccae27", "version": "38.00.000", "uri": "../flows/1421caa0-679d-4bf4-b282-0eb850ccae27.xml"}, "exchange direction": "INPUT", "meanAmount": 0.0, "other": {"anies": [{"value": "1.77E-4", "module": "A1", "scenario": "Standard scenario"}, {"value": "0.0", "module": "A2", "scenario": "Standard scenario"}, {"value": "2.67E-4", "module": "A3", "scenario": "Standard scenario"}, {"value": "2.67E-4", "module": "C1", "scenario": "Standard scenario"}, {"value": "2.67E-4", "module": "C2", "scenario": "Standard scenario"}, {"value": "-2.8E-14", "module": "C3", "scenario": "Standard scenario"}, {"value": "-4.0E-15", "module": "C4", "scenario": "Standard scenario"}, {"value": "-4.09E-13", "module": "D", "scenario": "Standard scenario"}, {"name": "referenceToUnitGroupDataSet", "value": {"shortDescription": [{"value": "MJ", "lang": "en"}], "type": "unit group data set", "refObjectId": "93a60a57-a3c8-11da-a746-0800200c9a66", "version": "03.00.000", "uri": "../unitgroups/93a60a57-a3c8-11da-a746-0800200c9a66.xml"}}]}, "flowProperties": [], "typeOfFlow": "Other flow", "classification": {"classHierarchy": "Quantities", "name": "GaBiCategories"}}, {"dataSetInternalID": 13, "referenceToFlowDataSet": {"shortDescription": [{"value": "Total use of non-renewable primary energy resources (PENRT)", "lang": "en"}, {"value": "Total nicht erneuerbare Primärenergie (PENRT)", "lang": "de"}, {"value": "Uso total de la energía primaria no renovable (energía primaria y recursos de energía primaria renovable utilizada como materia prima) (PENRT)", "lang": "es"}], "type": "flow data set", "refObjectId": "06159210-646b-4c8d-8583-da9b3b95a6c1", "version": "30.00.000", "uri": "../flows/06159210-646b-4c8d-8583-da9b3b95a6c1.xml"}, "exchange direction": "INPUT", "meanAmount": 0.0, "other": {"anies": [{"value": "208.0", "module": "A1", "scenario": "Standard scenario"}, {"value": "10.6", "module": "A2", "scenario": "Standard scenario"}, {"value": "7.06", "module": "A3", "scenario": "Standard scenario"}, {"value": "2.14", "module": "C1", "scenario": "Standard scenario"}, {"value": "0.214", "module": "C2", "scenario": "Standard scenario"}, {"value": "1.35", "module": "C3", "scenario": "Standard scenario"}, {"value": "0.766", "module": "C4", "scenario": "Standard scenario"}, {"value": "-55.8", "module": "D", "scenario": "Standard scenario"}, {"name": "referenceToUnitGroupDataSet", "value": {"shortDescription": [{"value": "MJ", "lang": "en"}], "type": "unit group data set", "refObjectId": "93a60a57-a3c8-11da-a746-0800200c9a66", "version": "03.00.000", "uri": "../unitgroups/93a60a57-a3c8-11da-a746-0800200c9a66.xml"}}]}, "flowProperties": [], "typeOfFlow": "Other flow", "classification": {"classHierarchy": "Größen / Umweltliche Größen / EPD EN 15804 / LCI Indikatoren", "name": "GaBiCategories"}}, {"dataSetInternalID": 14, "referenceToFlowDataSet": {"shortDescription": [{"value": "Use of renewable primary energy (PERE)", "lang": "en"}, {"value": "Erneuerbare Primärenergie als Energieträger (PERE)", "lang": "de"}, {"value": "Uso de energía primaria renovable excluyendo los recursos de energía primaria renovable utilizada como materia prima (PERE)", "lang": "es"}], "type": "flow data set", "refObjectId": "20f32be5-0398-4288-9b6d-accddd195317", "version": "38.00.000", "uri": "../flows/20f32be5-0398-4288-9b6d-accddd195317.xml"}, "exchange direction": "INPUT", "meanAmount": 0.0, "other": {"anies": [{"value": "35.3", "module": "A1", "scenario": "Standard scenario"}, {"value": "0.332", "module": "A2", "scenario": "Standard scenario"}, {"value": "3.15", "module": "A3", "scenario": "Standard scenario"}, {"value": "0.232", "module": "C1", "scenario": "Standard scenario"}, {"value": "0.0181", "module": "C2", "scenario": "Standard scenario"}, {"value": "0.952", "module": "C3", "scenario": "Standard scenario"}, {"value": "0.134", "module": "C4", "scenario": "Standard scenario"}, {"value": "-26.1", "module": "D", "scenario": "Standard scenario"}, {"name": "referenceToUnitGroupDataSet", "value": {"shortDescription": [{"value": "MJ", "lang": "en"}], "type": "unit group data set", "refObjectId": "93a60a57-a3c8-11da-a746-0800200c9a66", "version": "03.00.000", "uri": "../unitgroups/93a60a57-a3c8-11da-a746-0800200c9a66.xml"}}]}, "flowProperties": [], "typeOfFlow": "Other flow", "classification": {"classHierarchy": "Quantities", "name": "GaBiCategories"}}, {"dataSetInternalID": 15, "referenceToFlowDataSet": {"shortDescription": [{"value": "Use of renewable primary energy resources used as raw materials (PERM)", "lang": "en"}, {"value": "Erneuerbare Primärenergie zur stofflichen Nutzung (PERM)", "lang": "de"}, {"value": "Uso de energía primaria renovable utilizada como materia prima (PERM)", "lang": "es"}], "type": "flow data set", "refObjectId": "fb3ec0de-548d-4508-aea5-00b73bf6f702", "version": "38.00.000", "uri": "../flows/fb3ec0de-548d-4508-aea5-00b73bf6f702.xml"}, "exchange direction": "INPUT", "meanAmount": 0.0, "other": {"anies": [{"value": "1.77E-4", "module": "A1", "scenario": "Standard scenario"}, {"value": "0.0", "module": "A2", "scenario": "Standard scenario"}, {"value": "2.67E-4", "module": "A3", "scenario": "Standard scenario"}, {"value": "2.67E-4", "module": "C1", "scenario": "Standard scenario"}, {"value": "2.67E-4", "module": "C2", "scenario": "Standard scenario"}, {"value": "-2.8E-14", "module": "C3", "scenario": "Standard scenario"}, {"value": "-4.0E-15", "module": "C4", "scenario": "Standard scenario"}, {"value": "-4.09E-13", "module": "D", "scenario": "Standard scenario"}, {"name": "referenceToUnitGroupDataSet", "value": {"shortDescription": [{"value": "MJ", "lang": "en"}], "type": "unit group data set", "refObjectId": "93a60a57-a3c8-11da-a746-0800200c9a66", "version": "03.00.000", "uri": "../unitgroups/93a60a57-a3c8-11da-a746-0800200c9a66.xml"}}]}, "flowProperties": [], "typeOfFlow": "Other flow", "classification": {"classHierarchy": "Quantities", "name": "GaBiCategories"}}, {"dataSetInternalID": 16, "referenceToFlowDataSet": {"shortDescription": [{"value": "Total use of renewable primary energy resources (PERT)", "lang": "en"}, {"value": "Total erneuerbare Primärenergie (PERT)", "lang": "de"}, {"value": "Uso total de la energía primaria renovable (energía primaria y recursos de energía primaria renovable utilizada como materia prima) (PERT)", "lang": "es"}], "type": "flow data set", "refObjectId": "53f97275-fa8a-4cdd-9024-65936002acd0", "version": "30.00.000", "uri": "../flows/53f97275-fa8a-4cdd-9024-65936002acd0.xml"}, "exchange direction": "INPUT", "meanAmount": 0.0, "other": {"anies": [{"value": "35.3", "module": "A1", "scenario": "Standard scenario"}, {"value": "0.332", "module": "A2", "scenario": "Standard scenario"}, {"value": "3.15", "module": "A3", "scenario": "Standard scenario"}, {"value": "0.232", "module": "C1", "scenario": "Standard scenario"}, {"value": "0.0181", "module": "C2", "scenario": "Standard scenario"}, {"value": "0.952", "module": "C3", "scenario": "Standard scenario"}, {"value": "0.134", "module": "C4", "scenario": "Standard scenario"}, {"value": "-26.1", "module": "D", "scenario": "Standard scenario"}, {"name": "referenceToUnitGroupDataSet", "value": {"shortDescription": [{"value": "MJ", "lang": "en"}], "type": "unit group data set", "refObjectId": "93a60a57-a3c8-11da-a746-0800200c9a66", "version": "03.00.000", "uri": "../unitgroups/93a60a57-a3c8-11da-a746-0800200c9a66.xml"}}]}, "flowProperties": [], "typeOfFlow": "Other flow", "classification": {"classHierarchy": "Größen / Umweltliche Größen / EPD EN 15804 / LCI Indikatoren", "name": "GaBiCategories"}}, {"dataSetInternalID": 17, "referenceToFlowDataSet": {"shortDescription": [{"value": "Use of renewable secondary fuels (RSF)", "lang": "en"}, {"value": "Erneuerbare Sekundärbrennstoffe (RSF)", "lang": "de"}, {"value": "Uso de combustibles secundarios renovables (RSF)", "lang": "es"}], "type": "flow data set", "refObjectId": "64333088-a55f-4aa2-9a31-c10b07816787", "version": "30.00.000", "uri": "../flows/64333088-a55f-4aa2-9a31-c10b07816787.xml"}, "exchange direction": "INPUT", "meanAmount": 0.0, "other": {"anies": [{"value": "0.0", "module": "A1", "scenario": "Standard scenario"}, {"value": "0.0", "module": "A2", "scenario": "Standard scenario"}, {"value": "0.0", "module": "A3", "scenario": "Standard scenario"}, {"value": "0.0", "module": "C1", "scenario": "Standard scenario"}, {"value": "0.0", "module": "C2", "scenario": "Standard scenario"}, {"value": "0.0", "module": "C3", "scenario": "Standard scenario"}, {"value": "0.0", "module": "C4", "scenario": "Standard scenario"}, {"value": "0.0", "module": "D", "scenario": "Standard scenario"}, {"name": "referenceToUnitGroupDataSet", "value": {"shortDescription": [{"value": "MJ", "lang": "en"}], "type": "unit group data set", "refObjectId": "93a60a57-a3c8-11da-a746-0800200c9a66", "version": "03.00.000", "uri": "../unitgroups/93a60a57-a3c8-11da-a746-0800200c9a66.xml"}}]}, "flowProperties": [], "typeOfFlow": "Other flow", "classification": {"classHierarchy": "Größen / Umweltliche Größen / EPD EN 15804 / LCI Indikatoren", "name": "GaBiCategories"}}, {"dataSetInternalID": 18, "referenceToFlowDataSet": {"shortDescription": [{"value": "Radioactive waste disposed (RWD)", "lang": "en"}, {"value": "Entsorgter radioaktiver Abfall (RWD)", "lang": "de"}, {"value": "Residuos radiactivos eliminados (RWD)", "lang": "es"}], "type": "flow data set", "refObjectId": "3449546e-52ad-4b39-b809-9fb77cea8ff6", "version": "30.00.000", "uri": "../flows/3449546e-52ad-4b39-b809-9fb77cea8ff6.xml"}, "exchange direction": "OUTPUT", "meanAmount": 0.0, "other": {"anies": [{"value": "0.00756", "module": "A1", "scenario": "Standard scenario"}, {"value": "7.96E-6", "module": "A2", "scenario": "Standard scenario"}, {"value": "5.8E-4", "module": "A3", "scenario": "Standard scenario"}, {"value": "2.89E-6", "module": "C1", "scenario": "Standard scenario"}, {"value": "2.76E-7", "module": "C2", "scenario": "Standard scenario"}, {"value": "8.42E-5", "module": "C3", "scenario": "Standard scenario"}, {"value": "7.92E-6", "module": "C4", "scenario": "Standard scenario"}, {"value": "-0.00493", "module": "D", "scenario": "Standard scenario"}, {"name": "referenceToUnitGroupDataSet", "value": {"shortDescription": [{"value": "kg", "lang": "en"}], "type": "unit group data set", "refObjectId": "ad38d542-3fe9-439d-9b95-2f5f7752acaf", "version": "30.00.000", "uri": "../unitgroups/ad38d542-3fe9-439d-9b95-2f5f7752acaf.xml"}}]}, "flowProperties": [], "typeOfFlow": "Other flow", "classification": {"classHierarchy": "Größen / Umweltliche Größen / EPD EN 15804 / LCI Indikatoren", "name": "GaBiCategories"}}, {"dataSetInternalID": 19, "referenceToFlowDataSet": {"shortDescription": [{"value": "Use of secondary material (SM)", "lang": "en"}, {"value": "Einsatz von Sekundärstoffen (SM)", "lang": "de"}, {"value": "Uso de materiales secundarios (SM)", "lang": "es"}], "type": "flow data set", "refObjectId": "c6a1f35f-2d09-4f54-8dfb-97e502e1ce92", "version": "30.00.000", "uri": "../flows/c6a1f35f-2d09-4f54-8dfb-97e502e1ce92.xml"}, "exchange direction": "INPUT", "meanAmount": 0.0, "other": {"anies": [{"value": "2.56", "module": "A1", "scenario": "Standard scenario"}, {"value": "0.0", "module": "A2", "scenario": "Standard scenario"}, {"value": "0.0", "module": "A3", "scenario": "Standard scenario"}, {"value": "0.0", "module": "C1", "scenario": "Standard scenario"}, {"value": "0.0", "module": "C2", "scenario": "Standard scenario"}, {"value": "0.0", "module": "C3", "scenario": "Standard scenario"}, {"value": "0.0", "module": "C4", "scenario": "Standard scenario"}, {"value": "0.0", "module": "D", "scenario": "Standard scenario"}, {"name": "referenceToUnitGroupDataSet", "value": {"shortDescription": [{"value": "kg", "lang": "en"}], "type": "unit group data set", "refObjectId": "ad38d542-3fe9-439d-9b95-2f5f7752acaf", "version": "30.00.000", "uri": "../unitgroups/ad38d542-3fe9-439d-9b95-2f5f7752acaf.xml"}}]}, "flowProperties": [], "typeOfFlow": "Other flow", "classification": {"classHierarchy": "Größen / Umweltliche Größen / EPD EN 15804 / LCI Indikatoren", "name": "GaBiCategories"}}]}, "LCIAResults": {"LCIAResult": [{"referenceToLCIAMethodDataSet": {"shortDescription": [{"value": "Abiotic depletion potential - non-fossil resources (ADPE)", "lang": "en"}, {"value": "Potenzial für die Verknappung abiotischer Ressourcen – nicht fossile Ressourcen (ADPE)", "lang": "de"}], "type": "LCIA method data set", "refObjectId": "b2ad6494-c78d-11e6-9d9d-cec0c932ce01", "version": "01.00.011", "uri": "../lciamethods/b2ad6494-c78d-11e6-9d9d-cec0c932ce01.xml"}, "meanAmount": 0.0, "other": {"anies": [{"value": "6.3E-6", "module": "A1", "scenario": "Standard scenario"}, {"value": "2.87E-8", "module": "A2", "scenario": "Standard scenario"}, {"value": "3.25E-7", "module": "A3", "scenario": "Standard scenario"}, {"value": "2.79E-8", "module": "C1", "scenario": "Standard scenario"}, {"value": "1.39E-9", "module": "C2", "scenario": "Standard scenario"}, {"value": "1.41E-8", "module": "C3", "scenario": "Standard scenario"}, {"value": "3.77E-9", "module": "C4", "scenario": "Standard scenario"}, {"value": "-1.13E-6", "module": "D", "scenario": "Standard scenario"}, {"name": "referenceToUnitGroupDataSet", "value": {"shortDescription": [{"value": "kg Sb-eq.", "lang": "en"}], "type": "unit group data set", "refObjectId": "54ccd2d9-a32a-4fc2-923d-f2c8c93e89d4", "version": "30.00.000", "uri": "../unitgroups/54ccd2d9-a32a-4fc2-923d-f2c8c93e89d4.xml"}}]}}, {"referenceToLCIAMethodDataSet": {"shortDescription": [{"value": "Abiotic depletion potential - fossil resources (ADPF)", "lang": "en"}, {"value": "Potenzial für die Verknappung abiotischer Ressourcen – fossile Brennstoffe (ADPF)", "lang": "de"}], "type": "LCIA method data set", "refObjectId": "b2ad6110-c78d-11e6-9d9d-cec0c932ce01", "version": "01.00.011", "uri": "../lciamethods/b2ad6110-c78d-11e6-9d9d-cec0c932ce01.xml"}, "meanAmount": 0.0, "other": {"anies": [{"value": "210.0", "module": "A1", "scenario": "Standard scenario"}, {"value": "10.7", "module": "A2", "scenario": "Standard scenario"}, {"value": "7.06", "module": "A3", "scenario": "Standard scenario"}, {"value": "2.14", "module": "C1", "scenario": "Standard scenario"}, {"value": "0.214", "module": "C2", "scenario": "Standard scenario"}, {"value": "1.35", "module": "C3", "scenario": "Standard scenario"}, {"value": "0.766", "module": "C4", "scenario": "Standard scenario"}, {"value": "-55.8", "module": "D", "scenario": "Standard scenario"}, {"name": "referenceToUnitGroupDataSet", "value": {"shortDescription": [{"value": "MJ", "lang": "en"}], "type": "unit group data set", "refObjectId": "93a60a57-a3c8-11da-a746-0800200c9a66", "version": "03.00.000", "uri": "../unitgroups/93a60a57-a3c8-11da-a746-0800200c9a66.xml"}}]}}, {"referenceToLCIAMethodDataSet": {"shortDescription": [{"value": "Acidification potential, Accumulated Exceedance (AP)", "lang": "en"}, {"value": "Versauerungspotenzial, kumulierte Überschreitung (AP)", "lang": "de"}], "type": "LCIA method data set", "refObjectId": "b5c611c6-def3-11e6-bf01-fe55135034f3", "version": "01.03.010", "uri": "../lciamethods/b5c611c6-def3-11e6-bf01-fe55135034f3.xml"}, "meanAmount": 0.0, "other": {"anies": [{"value": "0.0325", "module": "A1", "scenario": "Standard scenario"}, {"value": "0.0189", "module": "A2", "scenario": "Standard scenario"}, {"value": "7.09E-4", "module": "A3", "scenario": "Standard scenario"}, {"value": "0.00166", "module": "C1", "scenario": "Standard scenario"}, {"value": "1.01E-4", "module": "C2", "scenario": "Standard scenario"}, {"value": "8.61E-4", "module": "C3", "scenario": "Standard scenario"}, {"value": "4.12E-4", "module": "C4", "scenario": "Standard scenario"}, {"value": "-0.0113", "module": "D", "scenario": "Standard scenario"}, {"name": "referenceToUnitGroupDataSet", "value": {"shortDescription": [{"value": "mol H+-eq.", "lang": "en"}], "type": "unit group data set", "refObjectId": "42e089ac-92bf-4bf2-8ca1-5fc40d18f2ed", "version": "00.01.000", "uri": "../unitgroups/42e089ac-92bf-4bf2-8ca1-5fc40d18f2ed.xml"}}]}}, {"referenceToLCIAMethodDataSet": {"shortDescription": [{"value": "Eutrophication potential - freshwater (EP-freshwater)", "lang": "en"}, {"value": "Eutrophierungspotenzial - Süßwasser (EP-freshwater)", "lang": "de"}], "type": "LCIA method data set", "refObjectId": "b53ec18f-7377-4ad3-86eb-cc3f4f276b2b", "version": "01.00.011", "uri": "../lciamethods/b53ec18f-7377-4ad3-86eb-cc3f4f276b2b.xml"}, "meanAmount": 0.0, "other": {"anies": [{"value": "9.25E-5", "module": "A1", "scenario": "Standard scenario"}, {"value": "1.29E-6", "module": "A2", "scenario": "Standard scenario"}, {"value": "7.0E-7", "module": "A3", "scenario": "Standard scenario"}, {"value": "4.43E-7", "module": "C1", "scenario": "Standard scenario"}, {"value": "6.99E-8", "module": "C2", "scenario": "Standard scenario"}, {"value": "4.17E-7", "module": "C3", "scenario": "Standard scenario"}, {"value": "1.32E-7", "module": "C4", "scenario": "Standard scenario"}, {"value": "-4.63E-6", "module": "D", "scenario": "Standard scenario"}, {"name": "referenceToUnitGroupDataSet", "value": {"shortDescription": [{"value": "kg P-eq.", "lang": "en"}], "type": "unit group data set", "refObjectId": "0429039d-a61d-4590-ba67-aa4a20a810a1", "version": "30.00.000", "uri": "../unitgroups/0429039d-a61d-4590-ba67-aa4a20a810a1.xml"}}]}}, {"referenceToLCIAMethodDataSet": {"shortDescription": [{"value": "Eutrophication potential - marine (EP-marine)", "lang": "en"}, {"value": "Eutrophierungspotenzial - Salzwasser (EP-marine)", "lang": "de"}], "type": "LCIA method data set", "refObjectId": "b5c619fa-def3-11e6-bf01-fe55135034f3", "version": "02.00.011", "uri": "../lciamethods/b5c619fa-def3-11e6-bf01-fe55135034f3.xml"}, "meanAmount": 0.0, "other": {"anies": [{"value": "0.00812", "module": "A1", "scenario": "Standard scenario"}, {"value": "0.00468", "module": "A2", "scenario": "Standard scenario"}, {"value": "2.09E-4", "module": "A3", "scenario": "Standard scenario"}, {"value": "8.09E-4", "module": "C1", "scenario": "Standard scenario"}, {"value": "4.95E-5", "module": "C2", "scenario": "Standard scenario"}, {"value": "2.66E-4", "module": "C3", "scenario": "Standard scenario"}, {"value": "1.06E-4", "module": "C4", "scenario": "Standard scenario"}, {"value": "-0.00188", "module": "D", "scenario": "Standard scenario"}, {"name": "referenceToUnitGroupDataSet", "value": {"shortDescription": [{"value": "kg N-eq.", "lang": "en"}], "type": "unit group data set", "refObjectId": "d05bb823-ecdf-4686-8c40-bf1d9257859f", "version": "00.00.003", "uri": "../unitgroups/d05bb823-ecdf-4686-8c40-bf1d9257859f.xml"}}]}}, {"referenceToLCIAMethodDataSet": {"shortDescription": [{"value": "Eutrophication potential - terrestrial (EP-terrestrial)", "lang": "en"}, {"value": "Eutrophierungspotenzial - Land (EP-terrestrial)", "lang": "de"}], "type": "LCIA method data set", "refObjectId": "b5c614d2-def3-11e6-bf01-fe55135034f3", "version": "01.02.010", "uri": "../lciamethods/b5c614d2-def3-11e6-bf01-fe55135034f3.xml"}, "meanAmount": 0.0, "other": {"anies": [{"value": "0.0875", "module": "A1", "scenario": "Standard scenario"}, {"value": "0.0514", "module": "A2", "scenario": "Standard scenario"}, {"value": "0.00223", "module": "A3", "scenario": "Standard scenario"}, {"value": "0.00894", "module": "C1", "scenario": "Standard scenario"}, {"value": "5.49E-4", "module": "C2", "scenario": "Standard scenario"}, {"value": "0.00399", "module": "C3", "scenario": "Standard scenario"}, {"value": "0.00117", "module": "C4", "scenario": "Standard scenario"}, {"value": "-0.0204", "module": "D", "scenario": "Standard scenario"}, {"name": "referenceToUnitGroupDataSet", "value": {"shortDescription": [{"value": "mol N-eq.", "lang": "en"}], "type": "unit group data set", "refObjectId": "71b4d617-0ec9-4d3f-b65e-e438940c2401", "version": "00.00.003", "uri": "../unitgroups/71b4d617-0ec9-4d3f-b65e-e438940c2401.xml"}}]}}, {"referenceToLCIAMethodDataSet": {"shortDescription": [{"value": "Potential Comparative Toxic Unit for ecosystems (ETP-fw)", "lang": "en"}, {"value": "Potenzielle Toxizitätsvergleichseinheit für Ökosysteme (ETP-fw)", "lang": "de"}], "type": "LCIA method data set", "refObjectId": "05316e7a-b254-4bea-9cf0-6bf33eb5c630", "version": "01.00.003", "uri": "../lciamethods/05316e7a-b254-4bea-9cf0-6bf33eb5c630.xml"}, "meanAmount": 0.0, "other": {"anies": [{"value": "70.5", "module": "A1", "scenario": "Standard scenario"}, {"value": "6.5", "module": "A2", "scenario": "Standard scenario"}, {"value": "1.99", "module": "A3", "scenario": "Standard scenario"}, {"value": "1.74", "module": "C1", "scenario": "Standard scenario"}, {"value": "0.157", "module": "C2", "scenario": "Standard scenario"}, {"value": "0.509", "module": "C3", "scenario": "Standard scenario"}, {"value": "0.441", "module": "C4", "scenario": "Standard scenario"}, {"value": "-11.4", "module": "D", "scenario": "Standard scenario"}, {"name": "referenceToUnitGroupDataSet", "value": {"shortDescription": [{"value": "CTUe", "lang": "en"}], "type": "unit group data set", "refObjectId": "aa959ded-f1eb-4efb-9c5c-2d60be36b3e6", "version": "00.00.003", "uri": "../unitgroups/aa959ded-f1eb-4efb-9c5c-2d60be36b3e6.xml"}}]}}, {"referenceToLCIAMethodDataSet": {"shortDescription": [{"value": "Global Warming Potential - biogenic (GWP-biogenic)", "lang": "en"}, {"value": "Globales Erwärmungspotenzial - biogen (GWP-biogenic)", "lang": "de"}], "type": "LCIA method data set", "refObjectId": "a7ea186c-9749-11ed-a8fc-0242ac120002", "version": "01.00.006", "uri": "../lciamethods/a7ea186c-9749-11ed-a8fc-0242ac120002.xml"}, "meanAmount": 0.0, "other": {"anies": [{"value": "0.00618", "module": "A1", "scenario": "Standard scenario"}, {"value": "-0.00701", "module": "A2", "scenario": "Standard scenario"}, {"value": "-0.18", "module": "A3", "scenario": "Standard scenario"}, {"value": "-0.012", "module": "C1", "scenario": "Standard scenario"}, {"value": "-1.4E-4", "module": "C2", "scenario": "Standard scenario"}, {"value": "8.2E-4", "module": "C3", "scenario": "Standard scenario"}, {"value": "-3.99E-4", "module": "C4", "scenario": "Standard scenario"}, {"value": "-0.0172", "module": "D", "scenario": "Standard scenario"}, {"name": "referenceToUnitGroupDataSet", "value": {"shortDescription": [{"value": "kg CO2-eq.", "lang": "en"}], "type": "unit group data set", "refObjectId": "1ebf3012-d0db-4de2-aefd-ef30cedb0be1", "version": "30.00.000", "uri": "../unitgroups/1ebf3012-d0db-4de2-aefd-ef30cedb0be1.xml"}}]}}, {"referenceToLCIAMethodDataSet": {"shortDescription": [{"value": "Global Warming Potential - fossil fuels (GWP-fossil)", "lang": "en"}, {"value": "Globales Erwärmungspotenzial - fossil (GWP-fossil)", "lang": "de"}], "type": "LCIA method data set", "refObjectId": "a7ea19c0-9749-11ed-a8fc-0242ac120002", "version": "01.00.009", "uri": "../lciamethods/a7ea19c0-9749-11ed-a8fc-0242ac120002.xml"}, "meanAmount": 0.0, "other": {"anies": [{"value": "10.2", "module": "A1", "scenario": "Standard scenario"}, {"value": "0.842", "module": "A2", "scenario": "Standard scenario"}, {"value": "0.51", "module": "A3", "scenario": "Standard scenario"}, {"value": "0.176", "module": "C1", "scenario": "Standard scenario"}, {"value": "0.0162", "module": "C2", "scenario": "Standard scenario"}, {"value": "2.72", "module": "C3", "scenario": "Standard scenario"}, {"value": "0.0581", "module": "C4", "scenario": "Standard scenario"}, {"value": "-3.78", "module": "D", "scenario": "Standard scenario"}, {"name": "referenceToUnitGroupDataSet", "value": {"shortDescription": [{"value": "kg CO2-eq.", "lang": "en"}], "type": "unit group data set", "refObjectId": "1ebf3012-d0db-4de2-aefd-ef30cedb0be1", "version": "30.00.000", "uri": "../unitgroups/1ebf3012-d0db-4de2-aefd-ef30cedb0be1.xml"}}]}}, {"referenceToLCIAMethodDataSet": {"shortDescription": [{"value": "Global Warming Potential - land use and land use change (GWP-luluc)", "lang": "en"}, {"value": "Globales Erwärmungspotenzial - luluc (GWP-luluc)", "lang": "de"}], "type": "LCIA method data set", "refObjectId": "a7ea1ae2-9749-11ed-a8fc-0242ac120002", "version": "01.00.006", "uri": "../lciamethods/a7ea1ae2-9749-11ed-a8fc-0242ac120002.xml"}, "meanAmount": 0.0, "other": {"anies": [{"value": "0.0031", "module": "A1", "scenario": "Standard scenario"}, {"value": "0.00468", "module": "A2", "scenario": "Standard scenario"}, {"value": "4.92E-4", "module": "A3", "scenario": "Standard scenario"}, {"value": "0.00316", "module": "C1", "scenario": "Standard scenario"}, {"value": "2.75E-4", "module": "C2", "scenario": "Standard scenario"}, {"value": "5.42E-5", "module": "C3", "scenario": "Standard scenario"}, {"value": "3.49E-4", "module": "C4", "scenario": "Standard scenario"}, {"value": "-7.65E-4", "module": "D", "scenario": "Standard scenario"}, {"name": "referenceToUnitGroupDataSet", "value": {"shortDescription": [{"value": "kg CO2-eq.", "lang": "en"}], "type": "unit group data set", "refObjectId": "1ebf3012-d0db-4de2-aefd-ef30cedb0be1", "version": "30.00.000", "uri": "../unitgroups/1ebf3012-d0db-4de2-aefd-ef30cedb0be1.xml"}}]}}, {"referenceToLCIAMethodDataSet": {"shortDescription": [{"value": "Global Warming Potential - total (GWP-total)", "lang": "en"}, {"value": "Globales Erwärmungspotenzial - total (GWP-total)", "lang": "de"}], "type": "LCIA method data set", "refObjectId": "a7ea142a-9749-11ed-a8fc-0242ac120002", "version": "04.00.017", "uri": "../lciamethods/a7ea142a-9749-11ed-a8fc-0242ac120002.xml"}, "meanAmount": 0.0, "other": {"anies": [{"value": "10.2", "module": "A1", "scenario": "Standard scenario"}, {"value": "0.84", "module": "A2", "scenario": "Standard scenario"}, {"value": "0.33", "module": "A3", "scenario": "Standard scenario"}, {"value": "0.167", "module": "C1", "scenario": "Standard scenario"}, {"value": "0.0164", "module": "C2", "scenario": "Standard scenario"}, {"value": "2.72", "module": "C3", "scenario": "Standard scenario"}, {"value": "0.0581", "module": "C4", "scenario": "Standard scenario"}, {"value": "-3.8", "module": "D", "scenario": "Standard scenario"}, {"name": "referenceToUnitGroupDataSet", "value": {"shortDescription": [{"value": "kg CO2-eq.", "lang": "en"}], "type": "unit group data set", "refObjectId": "1ebf3012-d0db-4de2-aefd-ef30cedb0be1", "version": "30.00.000", "uri": "../unitgroups/1ebf3012-d0db-4de2-aefd-ef30cedb0be1.xml"}}]}}, {"referenceToLCIAMethodDataSet": {"shortDescription": [{"value": "Potential Comparative Toxic Unit for humans - cancer effects (HTP-c)", "lang": "en"}, {"value": "Potenzielle Toxizitätsvergleichseinheit für den Menschen - kanzerogene Wirkung (HTP-c)", "lang": "de"}], "type": "LCIA method data set", "refObjectId": "2299222a-bbd8-474f-9d4f-4dd1f18aea7c", "version": "01.00.004", "uri": "../lciamethods/2299222a-bbd8-474f-9d4f-4dd1f18aea7c.xml"}, "meanAmount": 0.0, "other": {"anies": [{"value": "5.61E-9", "module": "A1", "scenario": "Standard scenario"}, {"value": "1.17E-10", "module": "A2", "scenario": "Standard scenario"}, {"value": "3.3E-9", "module": "A3", "scenario": "Standard scenario"}, {"value": "4.0E-11", "module": "C1", "scenario": "Standard scenario"}, {"value": "3.16E-12", "module": "C2", "scenario": "Standard scenario"}, {"value": "4.22E-11", "module": "C3", "scenario": "Standard scenario"}, {"value": "1.04E-11", "module": "C4", "scenario": "Standard scenario"}, {"value": "-9.18E-10", "module": "D", "scenario": "Standard scenario"}, {"name": "referenceToUnitGroupDataSet", "value": {"shortDescription": [{"value": "CTUh", "lang": "en"}], "type": "unit group data set", "refObjectId": "d4c9523e-2d7e-49fd-8469-998f547d3a70", "version": "00.00.003", "uri": "../unitgroups/d4c9523e-2d7e-49fd-8469-998f547d3a70.xml"}}]}}, {"referenceToLCIAMethodDataSet": {"shortDescription": [{"value": "Potential Comparative Toxic Unit for humans - non-cancer effects (HTP-nc)", "lang": "en"}, {"value": "Potenzielle Toxizitätsvergleichseinheit für den Menschen - nicht kanzerogene Wirkung (HTP-nc)", "lang": "de"}], "type": "LCIA method data set", "refObjectId": "7cfdcfcf-b222-4b26-888a-a55f9fbf7ac8", "version": "01.00.003", "uri": "../lciamethods/7cfdcfcf-b222-4b26-888a-a55f9fbf7ac8.xml"}, "meanAmount": 0.0, "other": {"anies": [{"value": "1.33E-7", "module": "A1", "scenario": "Standard scenario"}, {"value": "3.96E-9", "module": "A2", "scenario": "Standard scenario"}, {"value": "2.52E-9", "module": "A3", "scenario": "Standard scenario"}, {"value": "1.43E-9", "module": "C1", "scenario": "Standard scenario"}, {"value": "1.41E-10", "module": "C2", "scenario": "Standard scenario"}, {"value": "1.48E-9", "module": "C3", "scenario": "Standard scenario"}, {"value": "4.03E-10", "module": "C4", "scenario": "Standard scenario"}, {"value": "-2.29E-8", "module": "D", "scenario": "Standard scenario"}, {"name": "referenceToUnitGroupDataSet", "value": {"shortDescription": [{"value": "CTUh", "lang": "en"}], "type": "unit group data set", "refObjectId": "d4c9523e-2d7e-49fd-8469-998f547d3a70", "version": "00.00.003", "uri": "../unitgroups/d4c9523e-2d7e-49fd-8469-998f547d3a70.xml"}}]}}, {"referenceToLCIAMethodDataSet": {"shortDescription": [{"value": "Potential Human exposure efficiency relative to U235 (IRP)", "lang": "en"}, {"value": "Potenzielle Wirkung durch Exposition des Menschen mit U235 (IRP)", "lang": "de"}], "type": "LCIA method data set", "refObjectId": "b5c632be-def3-11e6-bf01-fe55135034f3", "version": "01.00.012", "uri": "../lciamethods/b5c632be-def3-11e6-bf01-fe55135034f3.xml"}, "meanAmount": 0.0, "other": {"anies": [{"value": "1.38", "module": "A1", "scenario": "Standard scenario"}, {"value": "0.00113", "module": "A2", "scenario": "Standard scenario"}, {"value": "0.0471", "module": "A3", "scenario": "Standard scenario"}, {"value": "2.95E-4", "module": "C1", "scenario": "Standard scenario"}, {"value": "3.86E-5", "module": "C2", "scenario": "Standard scenario"}, {"value": "0.00892", "module": "C3", "scenario": "Standard scenario"}, {"value": "9.03E-4", "module": "C4", "scenario": "Standard scenario"}, {"value": "-0.926", "module": "D", "scenario": "Standard scenario"}, {"name": "referenceToUnitGroupDataSet", "value": {"shortDescription": [{"value": "kgBq U235-eq.", "lang": "en"}], "type": "unit group data set", "refObjectId": "456b05bf-1415-44a9-9993-02452f554c09", "version": "00.00.003", "uri": "../unitgroups/456b05bf-1415-44a9-9993-02452f554c09.xml"}}]}}, {"referenceToLCIAMethodDataSet": {"shortDescription": [{"value": "Depletion potential of the stratospheric ozone layer (ODP)", "lang": "en"}, {"value": "Abbaupotenzial der stratosphärischen Ozonschicht (ODP)", "lang": "de"}], "type": "LCIA method data set", "refObjectId": "b5c629d6-def3-11e6-bf01-fe55135034f3", "version": "02.00.013", "uri": "../lciamethods/b5c629d6-def3-11e6-bf01-fe55135034f3.xml"}, "meanAmount": 0.0, "other": {"anies": [{"value": "1.68E-8", "module": "A1", "scenario": "Standard scenario"}, {"value": "8.68E-14", "module": "A2", "scenario": "Standard scenario"}, {"value": "3.59E-10", "module": "A3", "scenario": "Standard scenario"}, {"value": "3.84E-14", "module": "C1", "scenario": "Standard scenario"}, {"value": "1.65E-15", "module": "C2", "scenario": "Standard scenario"}, {"value": "2.03E-12", "module": "C3", "scenario": "Standard scenario"}, {"value": "1.58E-13", "module": "C4", "scenario": "Standard scenario"}, {"value": "-3.92E-11", "module": "D", "scenario": "Standard scenario"}, {"name": "referenceToUnitGroupDataSet", "value": {"shortDescription": [{"value": "kg CFC-11-eq.", "lang": "en"}], "type": "unit group data set", "refObjectId": "d9e957c9-7309-4474-bf3a-7777df6c4e5b", "version": "25.00.000", "uri": "../unitgroups/d9e957c9-7309-4474-bf3a-7777df6c4e5b.xml"}}]}}, {"referenceToLCIAMethodDataSet": {"shortDescription": [{"value": "Potential incidence of disease due to PM emissions (PM)", "lang": "en"}, {"value": "Potenzielles Auftreten von Krankheiten aufgrund von Feinstaubemissionen (PM)", "lang": "de"}], "type": "LCIA method data set", "refObjectId": "b5c602c6-def3-11e6-bf01-fe55135034f3", "version": "02.00.012", "uri": "../lciamethods/b5c602c6-def3-11e6-bf01-fe55135034f3.xml"}, "meanAmount": 0.0, "other": {"anies": [{"value": "6.09E-7", "module": "A1", "scenario": "Standard scenario"}, {"value": "3.36E-7", "module": "A2", "scenario": "Standard scenario"}, {"value": "2.87E-8", "module": "A3", "scenario": "Standard scenario"}, {"value": "4.9E-8", "module": "C1", "scenario": "Standard scenario"}, {"value": "6.47E-10", "module": "C2", "scenario": "Standard scenario"}, {"value": "4.93E-9", "module": "C3", "scenario": "Standard scenario"}, {"value": "5.17E-9", "module": "C4", "scenario": "Standard scenario"}, {"value": "-1.7E-7", "module": "D", "scenario": "Standard scenario"}, {"name": "referenceToUnitGroupDataSet", "value": {"shortDescription": [{"value": "Disease incidence", "lang": "en"}], "type": "unit group data set", "refObjectId": "3883559b-648f-4afc-8ba2-0bd24f3affa3", "version": "00.00.003", "uri": "../unitgroups/3883559b-648f-4afc-8ba2-0bd24f3affa3.xml"}}]}}, {"referenceToLCIAMethodDataSet": {"shortDescription": [{"value": "Photochemical Ozone Creation Potential (POCP)", "lang": "en"}, {"value": "Bildungspotenzial für troposphärisches Ozon (POCP)", "lang": "de"}], "type": "LCIA method data set", "refObjectId": "b5c610fe-def3-11e6-bf01-fe55135034f3", "version": "02.00.015", "uri": "../lciamethods/b5c610fe-def3-11e6-bf01-fe55135034f3.xml"}, "meanAmount": 0.0, "other": {"anies": [{"value": "0.0258", "module": "A1", "scenario": "Standard scenario"}, {"value": "0.0133", "module": "A2", "scenario": "Standard scenario"}, {"value": "5.78E-4", "module": "A3", "scenario": "Standard scenario"}, {"value": "0.00239", "module": "C1", "scenario": "Standard scenario"}, {"value": "9.48E-5", "module": "C2", "scenario": "Standard scenario"}, {"value": "6.9E-4", "module": "C3", "scenario": "Standard scenario"}, {"value": "3.25E-4", "module": "C4", "scenario": "Standard scenario"}, {"value": "-0.00559", "module": "D", "scenario": "Standard scenario"}, {"name": "referenceToUnitGroupDataSet", "value": {"shortDescription": [{"value": "kg NMVOC-eq.", "lang": "en"}], "type": "unit group data set", "refObjectId": "d27c25f8-fbc1-44c6-b47b-4adbae4199c6", "version": "00.00.003", "uri": "../unitgroups/d27c25f8-fbc1-44c6-b47b-4adbae4199c6.xml"}}]}}, {"referenceToLCIAMethodDataSet": {"shortDescription": [{"value": "Potential Soil quality index (SQP)", "lang": "en"}, {"value": "Potenzieller Bodenqualitätsindex (SQP)", "lang": "de"}], "type": "LCIA method data set", "refObjectId": "b2ad6890-c78d-11e6-9d9d-cec0c932ce01", "version": "01.00.011", "uri": "../lciamethods/b2ad6890-c78d-11e6-9d9d-cec0c932ce01.xml"}, "meanAmount": 0.0, "other": {"anies": [{"value": "17.8", "module": "A1", "scenario": "Standard scenario"}, {"value": "1.81", "module": "A2", "scenario": "Standard scenario"}, {"value": "33.0", "module": "A3", "scenario": "Standard scenario"}, {"value": "1.43", "module": "C1", "scenario": "Standard scenario"}, {"value": "0.106", "module": "C2", "scenario": "Standard scenario"}, {"value": "0.692", "module": "C3", "scenario": "Standard scenario"}, {"value": "0.218", "module": "C4", "scenario": "Standard scenario"}, {"value": "-6.21", "module": "D", "scenario": "Standard scenario"}, {"name": "referenceToUnitGroupDataSet", "value": {"shortDescription": [{"value": "dimensionless", "lang": "en"}], "type": "unit group data set", "refObjectId": "f130951c-e67f-4f7f-8dd4-665de3974e18", "version": "00.00.004", "uri": "../unitgroups/f130951c-e67f-4f7f-8dd4-665de3974e18.xml"}}]}}, {"referenceToLCIAMethodDataSet": {"shortDescription": [{"value": "Water (user) deprivation potential (WDP)", "lang": "en"}, {"value": "Wasser-Entzugspotenzial (Benutzer) (WDP)", "lang": "de"}], "type": "LCIA method data set", "refObjectId": "b2ad66ce-c78d-11e6-9d9d-cec0c932ce01", "version": "03.00.015", "uri": "../lciamethods/b2ad66ce-c78d-11e6-9d9d-cec0c932ce01.xml"}, "meanAmount": 0.0, "other": {"anies": [{"value": "1.16", "module": "A1", "scenario": "Standard scenario"}, {"value": "0.00474", "module": "A2", "scenario": "Standard scenario"}, {"value": "0.0381", "module": "A3", "scenario": "Standard scenario"}, {"value": "0.00116", "module": "C1", "scenario": "Standard scenario"}, {"value": "2.44E-4", "module": "C2", "scenario": "Standard scenario"}, {"value": "0.275", "module": "C3", "scenario": "Standard scenario"}, {"value": "0.00663", "module": "C4", "scenario": "Standard scenario"}, {"value": "-0.129", "module": "D", "scenario": "Standard scenario"}, {"name": "referenceToUnitGroupDataSet", "value": {"shortDescription": [{"value": "m3 world eq. deprived", "lang": "en"}], "type": "unit group data set", "refObjectId": "6ae2df01-888e-46c8-b17d-49fa3869b476", "version": "00.00.003", "uri": "../unitgroups/6ae2df01-888e-46c8-b17d-49fa3869b476.xml"}}]}}]}, "otherAttributes": {"{http://www.indata.network/EPD/2019}epd-version": "1.2", "{http://www.okworx.com/ILCD/Extensions/2018/Profile}profile": "EN_15804_A2"}, "version": "1.1"}