{"processInformation": {"dataSetInformation": {"UUID": "1fe648df-fd53-4231-b43d-fcf26b20978a", "name": {"baseName": [{"value": "Unilin Medium Density Fiberboard", "lang": "en"}, {"value": "Unilin Medium Density Fiberboard", "lang": "de"}], "functionalUnitFlowProperties": [{"lang": "en"}]}, "classificationInformation": {"classification": [{"class": [{"value": "Holz", "level": 0, "classId": "3"}, {"value": "Holzwerkstoffe", "level": 1, "classId": "3.2"}, {"value": "Holzfaserplatten", "level": 2, "classId": "3.2.07"}], "name": "OEKOBAU.DAT"}, {"class": [{"value": "02 Building products", "level": 0}, {"value": "Wood based panels", "level": 1}, {"value": "Wood-based panels", "level": 2}], "name": "IBUCategories"}]}, "generalComment": [{"value": "A medium density fiberboard is a versatile engineered wood product designed for various applications. It is generated by compressing wood fibers and glue under high pressure and temperature, resulting in a smooth, homogeneous panel with excellent strength and dimensional stability.", "lang": "en"}, {"value": "Eine mitteldichte Faserplatte ist ein vielseitiger Holzwerkstoff, der für verschiedene Anwendungen entwickelt wurde. Sie wird durch Komprimierung von Holzfasern und Leim unter hohem Druck und hoher Temperatur hergestellt. Das Ergebnis ist eine glatte, homogene Platte mit ausgezeichneter Festigkeit und Dimensionsstabilität.", "lang": "de"}]}, "quantitativeReference": {"referenceToReferenceFlow": [0]}, "time": {"referenceYear": 2023, "dataSetValidUntil": 2028, "other": {"anies": [{"name": "publicationDateOfEPD", "value": 1698710400000}]}}, "geography": {"locationOfOperationSupplyOrProduction": {"location": "WEU"}}, "technology": {"technologyDescriptionAndIncludedProcesses": [{"value": "Round wood is collected to produce the fiberboards. The bark is removed from the round wood logs. The logs are chopped to wood chips. The wood chips are defibrated under high pressure in a refiner. The board is produced by introducing the fibermat into a press, which compresses it under higher pressure and temperature. The board is sanded, cut into panels and finished depending on the intended application. \nTechnical data: \nTechnical characteristics vary by product variant and thickness. More detailed product-specific data, technical data sheets and the CE declaration of performance are available on www.unilinpanels.com. \nDeclared unit: \nThe declared information and values refer to 1 m of Unilin MDF board with a sales-weighted average composition and density of 637 kg/m.", "lang": "en"}, {"value": "Für die Herstellung der Faserplatten wird Rundholz gesammelt.\nVon den Rundholzstämmen wird die Rinde entfernt.\nDie Stämme werden zu Holzspänen zerkleinert.\nDie Holzspäne werden unter hohem Druck in einem Refiner zerfasert.\n\nDie Platte wird hergestellt, indem das Fasermaterial in eine Presse gegeben wird, die es unter höherem Druck und höherer Temperatur komprimiert.\nDie Platte wird geschliffen, in Platten geschnitten und je nach Verwendungszweck bearbeitet. \nTechnische Daten: \nDie technischen Eigenschaften variieren je nach Produktvariante und Dicke. Ausführlichere produktspezifische Daten, technische Datenblätter und die CE-Leistungserklärung finden Sie unter www.unilinpanels.com. \nDeklarierte Einheit: \nDie angegebenen Informationen und Werte beziehen sich auf 1 m³ Unilin MDF-Platte mit einer verkaufsgewichteten durchschnittlichen Zusammensetzung und Dichte von 637 kg/m³.", "lang": "de"}], "technologicalApplicability": [{"value": "Unilin's MDF boards are highly versatile and used in both structural and non-structural applications. The surface variety accommodates the use of a versatile range of finishes and coatings, making the material easy to use in many different designs and applications.\n\nThe product is predominantly used with a coated surface. Fiberboards are typically used in furniture as counters, worktops, displays, wall coverings. MDF boards are also suitable for manufacturing doors and frames (coated, foiled, painted) and can be milled due to their homogeneous structure.\n\nUnilin Fiberboards can be used in a variety of applications, classified according EN 622-5:2010 :\nMDF : General purpose boards for use in dry conditions\n\nMDF.H : General purpose boards for use in humid conditions \nMDF.LA : Load-bearing boards for use in dry conditions \nMDF.HLS : Load-bearing boards for use in humid conditions\nL-MDF : Light MDF boards for use in dry conditions\nL-MDF.H : Light MDF boards for use in humid conditions \nUL1-MDF : Ultra-light MDF boards for use in dry conditions \nUL2-MDF : Ultra-light MDF boards for use in dry conditions \nMDF.RWH : For use in rigid underlays in roofs and walls", "lang": "en"}, {"value": "Die MDF-Platten von Unilin sind äußerst vielseitig und werden sowohl für strukturelle als auch für nicht-strukturelle Anwendungen eingesetzt. Die Oberflächenvielfalt ermöglicht die Verwendung eines vielseitigen Spektrums an Veredelungen und Beschichtungen, so dass das Material leicht in vielen verschiedenen Designs und Anwendungen eingesetzt werden kann. Das Produkt wird überwiegend mit einer beschichteten Oberfläche verwendet. Faserplatten werden typischerweise in Möbeln als Theken, Arbeitsplatten, Displays und Wandverkleidungen verwendet. MDF-Platten eignen sich auch für die Herstellung von Türen und Rahmen (beschichtet, foliert, lackiert) und können aufgrund ihrer homogenen Struktur gefräst werden. Unilin Faserplatten können in einer Vielzahl von Anwendungen eingesetzt werden, klassifiziert nach EN 622-5:2010 : MDF : Platten für allgemeine Zwecke zur Verwendung unter trockenen Bedingungen MDF.H : Platten für allgemeine Zwecke zur Verwendung unter feuchten Bedingungen MDF.LA : Tragfähige Platten für den Einsatz unter trockenen Bedingungen MDF.HLS : Tragfähige Platten für den Einsatz unter feuchten Bedingungen L-MDF : Leichte MDF-Platten für den Einsatz unter trockenen Bedingungen L-MDF.H : Leichte MDF-Platten für den Einsatz unter feuchten Bedingungen UL1-MDF : Ultraleichte MDF-Platten für den Einsatz unter trockenen Bedingungen UL2-MDF : Ultraleichte MDF-Platten für den Einsatz unter trockenen Bedingungen MDF.RWH : Für den Einsatz in starren Unterkonstruktionen in Dach und Wand", "lang": "de"}]}}, "modellingAndValidation": {"LCIMethodAndAllocation": {"typeOfDataSet": "EPD", "referenceToLCAMethodDetails": [{"shortDescription": [{"value": "Wood-based panels.pdf", "lang": "en"}], "type": "source data set", "refObjectId": "f67e55c8-5d96-4fb2-bde2-d60e624326f5"}], "other": {"anies": [{"name": "subType", "value": "representative dataset"}]}}, "dataSourcesTreatmentAndRepresentativeness": {"referenceToDataSource": [{"shortDescription": [{"value": "ecoinvent database (all versions)", "lang": "en"}], "type": "source data set", "refObjectId": "b497a91f-e14b-4b69-8f28-f50eb1576766"}], "useAdviceForDataSet": [{"value": "Scope: \nThe scope of this EPD extends to Unilin's entire raw medium density fiberboard (MDF) range. The values declared refer to the sales-weighted average product. These are produced in following manufacturing sites:\n\nBazeilles, France\nVielsalm, Belgium \nSystem boundary: \nThis is a cradle-to-gate EPD with options, including the following life cycle phases A1 - A3, C1 - C4 and D. The following processes have been considered for each of the modules:\n\nA1 - A3: Product Stage\nThe production stage encompasses the extraction of raw materials (i.e. wood, glue, additives), their transportation to the production plants, and the subsequent manufacturing of the product. The required energy for production, ancillary materials, and production emissions are included. Energy and material input/output data were obtained from Unilin's fiberboard factories (Bazeilles and Vielsalm) as well as Unilin's glue factory.\n\nA large share of the used thermal energy is derived from renewable sources, such as internal and external woody waste streams. Any remaining energy needs are met through the local grid in Belgium or France.\n\nC1: Deconstruction/Demolition stage\nIt is assumed that the end-of-life fiberboard is manually dismantled from the building/furniture. The efforts involved in this process are considered negligible, leading to the absence of a declared environmental impact arising from the dismantling of the product.\n\nC2: Transport to Waste Processing\nThis life cycle stage describes the impact of the end-of-life product's transport from the demolition site to the waste processing facility. A representative distance of 50 km is assumed.\n\nC3: Waste Processing\nProcessing of the post-consumer MDF waste involves (preliminary) sorting and shredding of the material. The fiberboard is repurposed as a secondary fuel and undergoes energy recovery in module D. The material and its inherent properties (e.g. biogenic carbon and primary energy content) are thus exported from the system in C3.\n\nC4: Waste Disposal\nThis module describes the loads and emissions attributed to the disposal of the product after waste processing. As the end-of-life product leaves the system in C3 as a secondary fuel, no environmental impact is declared in C4.\n\nD: Loads and Benefits beyond the System Boundaries\nModule D describes the loads and benefits related to the use of the end-of-life MDF as a secondary fuel. This involves the energy recovery of post-consumer fiberboard waste, where it replaces a European-averaged mix of electricity and heat.\n\nThe system boundary between subsequent systems is defined in accordance with EN 15804+A2, i.e. when the material reaches its end-of-waste state. End-of-life fiberboard reaches its end-of-waste state after a sorting and shredding step, as inventoried in C3. The material leaves the current system at module C3 and enters a subsequent system as a secondary fuel.", "lang": "en"}, {"value": "Gültigkeitsbereich: \nDer Geltungsbereich dieser EPD erstreckt sich auf die gesamte Palette der mitteldichten Rohfaserplatten (MDF) von Unilin. Die angegebenen Werte beziehen sich auf das umsatzgewichtete Durchschnittsprodukt. Diese werden in folgenden Produktionsstätten hergestellt: Bazeilles, Frankreich Vielsalm, Belgien \nSystemgrenze: \nDies ist eine Cradle-to-Gate-EPD mit Optionen, die die folgenden Lebenszyklusphasen A1 - A3, C1 - C4 und D umfasst. Für jedes der Module wurden die folgenden Prozesse berücksichtigt: A1 - A3: Produktphase Die Produktionsphase umfasst die Gewinnung von Rohstoffen (z.B. Holz, Leim, Zusatzstoffe), deren Transport zu den Produktionsstätten und die anschließende Herstellung des Produkts. Die für die Produktion benötigte Energie, die Hilfsstoffe und die Produktionsemissionen werden einbezogen. Die Daten zum Energie- und Materialinput und -output stammen aus den Faserplattenwerken von Unilin (Bazeilles und Vielsalm) sowie aus der Leimfabrik von Unilin. Ein großer Teil der verwendeten Wärmeenergie stammt aus erneuerbaren Quellen wie internen und externen Holzabfallströmen. Der verbleibende Energiebedarf wird über das lokale Netz in Belgien oder Frankreich gedeckt. C1: Rückbau/Abbruchphase Es wird davon ausgegangen, dass die ausgedienten Faserplatten manuell vom Gebäude/Möbel abgebaut werden. Der mit diesem Prozess verbundene Aufwand wird als vernachlässigbar angesehen, so dass keine Umweltauswirkungen durch die Demontage des Produkts deklariert werden. C2: Transport zur Abfallverarbeitung Diese Lebenszyklusphase beschreibt die Auswirkungen des Transports des Altprodukts von der Abbruchstelle zur Abfallverarbeitungsanlage. Es wird von einer repräsentativen Entfernung von 50 km ausgegangen. C3: Abfallverarbeitung Die Verarbeitung des MDF-Abfalls umfasst das (vorläufige) Sortieren und Zerkleinern des Materials. Die Faserplatten werden als Sekundärbrennstoff wiederverwendet und in Modul D energetisch verwertet. Das Material und seine inhärenten Eigenschaften (z.B. biogener Kohlenstoff und Primärenergiegehalt) werden somit aus dem System in C3 exportiert. C4: Abfallentsorgung Dieses Modul beschreibt die Belastungen und Emissionen, die mit der Entsorgung des Produkts nach der Abfallverarbeitung verbunden sind. Da das End-of-Life-Produkt das System in C3 als Sekundärbrennstoff verlässt, werden in C4 keine Umweltauswirkungen angegeben. D: Belastungen und Nutzen über die Systemgrenzen hinaus Modul D beschreibt die Belastungen und den Nutzen im Zusammenhang mit der Verwendung der End-of-Life-MDF als Sekundärbrennstoff. Dabei handelt es sich um die energetische Verwertung von Post-Consumer-Faserplattenabfällen, wo sie einen europäischen Durchschnittsmix aus Strom und Wärme ersetzen. Die Systemgrenze zwischen den nachfolgenden Systemen wird gemäß EN 15804+A2 definiert, d.h. wenn das Material seinen End-of-Waste-Zustand erreicht. Altfaserplatten erreichen ihr Abfallende nach einem Sortier- und Zerkleinerungsschritt, wie in C3 inventarisiert. Das Material verlässt das aktuelle System am Modul C3 und gelangt als Sekundärbrennstoff in ein nachfolgendes System.", "lang": "de"}], "other": {"anies": [{"name": "referenceToOriginalEPD", "value": {"shortDescription": {"value": "Unilin Medium Density Fiberboard.pdf", "defaultValue": "Unilin Medium Density Fiberboard.pdf", "lstrings": [{"lang": "en", "value": "Unilin Medium Density Fiberboard.pdf"}]}, "type": "source data set", "uuid": {"uuid": "d2f3ab9a-3bee-44e8-b098-aaeeadc42a79"}, "refObjectId": "d2f3ab9a-3bee-44e8-b098-aaeeadc42a79", "resourceURLs": ["https://oekobaudat.de/OEKOBAU.DAT/resource/sources/d2f3ab9a-3bee-44e8-b098-aaeeadc42a79/Unilin_Medium_Density_Fiberboard_18275.pdf?version=00.01.000"]}}]}}, "validation": {"review": [{"referenceToNameOfReviewerAndInstitution": [{"shortDescription": [{"value": "Institut Bauen und Umwelt e. V.", "lang": "en"}], "type": "contact data set", "refObjectId": "d111dbec-b024-4be5-86c5-752d6eb2cf95", "uri": "../contacts/d111dbec-b024-4be5-86c5-752d6eb2cf95.xml"}], "type": "Accredited third party review"}]}, "complianceDeclarations": {"compliance": [{"referenceToComplianceSystem": {"shortDescription": [{"value": "DIN EN 15804+A2", "lang": "en"}], "type": "source data set", "refObjectId": "c0016b33-8cf7-415c-ac6e-deba0d21440d", "uri": "../sources/c0016b33-8cf7-415c-ac6e-deba0d21440d.xml"}}, {"referenceToComplianceSystem": {"shortDescription": [{"value": "ISO 14025", "lang": "en"}], "type": "source data set", "refObjectId": "4f2eb655-6e44-4874-a95a-e28f5442cd4d", "uri": "../sources/4f2eb655-6e44-4874-a95a-e28f5442cd4d.xml"}}]}}, "administrativeInformation": {"commissionerAndGoal": {"referenceToCommissioner": [{"shortDescription": [{"value": "Unilin B.V. Division Panels", "lang": "en"}], "type": "contact data set", "refObjectId": "ed0749a7-681d-40e4-be8b-488335dfffda", "uri": "../contacts/ed0749a7-681d-40e4-be8b-488335dfffda.xml"}]}, "dataGenerator": {"referenceToPersonOrEntityGeneratingTheDataSet": [{"shortDescription": [{"value": "Unilin B.V. Division Panels", "lang": "en"}], "type": "contact data set", "refObjectId": "ed0749a7-681d-40e4-be8b-488335dfffda", "uri": "../contacts/ed0749a7-681d-40e4-be8b-488335dfffda.xml"}]}, "dataEntryBy": {"timeStamp": 1698710400000, "referenceToDataSetFormat": [{"shortDescription": [{"value": "ILCD Format", "lang": "en"}], "type": "source data set", "refObjectId": "a97a0155-0234-4b87-b4ce-a45da52f2a40", "uri": "../sources/a97a0155-0234-4b87-b4ce-a45da52f2a40.xml"}, {"shortDescription": [{"value": "EPD-Datenformaterweiterungen v1.2", "lang": "de"}, {"value": "EPD Data Format Extensions v1.2", "lang": "en"}], "type": "source data set", "refObjectId": "a29449fd-aa2f-4de8-b5d7-4b06b43c6fde", "uri": "../sources/a29449fd-aa2f-4de8-b5d7-4b06b43c6fde.xml"}]}, "publicationAndOwnership": {"dataSetVersion": "00.02.000", "referenceToRegistrationAuthority": {"shortDescription": [{"value": "Institut Bauen und Umwelt e. V.", "lang": "en"}], "type": "contact data set", "refObjectId": "d111dbec-b024-4be5-86c5-752d6eb2cf95", "uri": "../contacts/d111dbec-b024-4be5-86c5-752d6eb2cf95.xml"}, "registrationNumber": "EPD-UNI-20230378-IBJ1-EN", "referenceToOwnershipOfDataSet": {"shortDescription": [{"value": "Unilin B.V. Division Panels", "lang": "en"}], "type": "contact data set", "refObjectId": "ed0749a7-681d-40e4-be8b-488335dfffda", "uri": "../contacts/ed0749a7-681d-40e4-be8b-488335dfffda.xml"}, "copyright": true, "licenseType": "Free of charge for all users and uses", "accessRestrictions": [{"value": "None", "lang": "en"}], "other": {"anies": [{"name": "referenceToPublisher", "value": {"shortDescription": [{"value": "Institut Bauen und Umwelt e. V.", "lang": "en"}], "type": "contact data set", "refObjectId": "d111dbec-b024-4be5-86c5-752d6eb2cf95", "uri": "../contacts/d111dbec-b024-4be5-86c5-752d6eb2cf95.xml"}}]}}}, "exchanges": {"exchange": [{"dataSetInternalID": 0, "referenceToFlowDataSet": {"shortDescription": [{"value": "Unilin MDF Board (Unilin Medium Density Fiberboard)", "lang": "en"}], "type": "flow data set", "refObjectId": "7e0547f9-8b2f-b1f4-2666-e9f9c592b860", "uri": "../flows/7e0547f9-8b2f-b1f4-2666-e9f9c592b860.xml"}, "meanAmount": 1.0, "referencesToDataSource": {}, "referenceFlow": true, "resolvedFlowVersion": "00.02.000", "resultingflowAmount": 1.0, "flowProperties": [{"name": [{"lang": "en", "value": "Volume"}, {"lang": "de", "value": "Volumen"}], "uuid": "93a60a56-a3c8-22da-a746-0800200c9a66", "referenceFlowProperty": true, "meanValue": 1.0, "referenceUnit": "m3", "unitGroupUUID": "cd950537-0a98-4044-9ba7-9f9a68d0a504"}], "materialProperties": [{"name": "gross density", "value": "637.0", "unit": "kg/m^3", "unitDescription": "kilograms per cubic metre"}], "typeOfFlow": "Product flow", "classification": {"classHierarchy": "Holz / Holzwerkstoffe / Holzfaserplatten", "name": "OEKOBAU.DAT"}}, {"dataSetInternalID": 1, "referenceToFlowDataSet": {"shortDescription": [{"value": "Renewable primary energy as energy carrier (PERE)", "lang": "en"}, {"value": "Erneuerbare Primärenergie als Energieträger (PERE)", "lang": "de"}], "type": "flow data set", "refObjectId": "20f32be5-0398-4288-9b6d-accddd195317", "uri": "../flows/20f32be5-0398-4288-9b6d-accddd195317.xml"}, "exchange direction": "INPUT", "other": {"anies": [{"name": "referenceToUnitGroupDataSet", "value": {"shortDescription": [{"value": "MJ", "lang": "en"}], "type": "unit group data set", "refObjectId": "93a60a57-a3c8-11da-a746-0800200c9a66", "uri": "../unitgroups/93a60a57-a3c8-11da-a746-0800200c9a66.xml"}}, {"value": "4705.01072822792", "module": "A1-A3"}, {"value": "0", "module": "C1"}, {"value": "0.573290680639056", "module": "C2"}, {"value": "9694.24911300666", "module": "C3"}, {"value": "0", "module": "C4"}, {"value": "-1204.76069363582", "module": "D"}]}, "resolvedFlowVersion": "38.00.000", "flowProperties": [], "typeOfFlow": "Other flow", "classification": {"classHierarchy": "Quantities", "name": "GaBiCategories"}}, {"dataSetInternalID": 2, "referenceToFlowDataSet": {"shortDescription": [{"value": "Renewable primary energy resources as material utilization (PERM)", "lang": "en"}, {"value": "Erneuerbare Primärenergie zur stofflichen Nutzung (PERM)", "lang": "de"}], "type": "flow data set", "refObjectId": "fb3ec0de-548d-4508-aea5-00b73bf6f702", "uri": "../flows/fb3ec0de-548d-4508-aea5-00b73bf6f702.xml"}, "exchange direction": "INPUT", "other": {"anies": [{"name": "referenceToUnitGroupDataSet", "value": {"shortDescription": [{"value": "MJ", "lang": "en"}], "type": "unit group data set", "refObjectId": "93a60a57-a3c8-11da-a746-0800200c9a66", "uri": "../unitgroups/93a60a57-a3c8-11da-a746-0800200c9a66.xml"}}, {"value": "9673.60118086744", "module": "A1-A3"}, {"value": "0", "module": "C1"}, {"value": "0", "module": "C2"}, {"value": "-9673.58", "module": "C3"}, {"value": "0", "module": "C4"}, {"value": "0", "module": "D"}]}, "resolvedFlowVersion": "38.00.000", "flowProperties": [], "typeOfFlow": "Other flow", "classification": {"classHierarchy": "Quantities", "name": "GaBiCategories"}}, {"dataSetInternalID": 3, "referenceToFlowDataSet": {"shortDescription": [{"value": "Total use of renewable primary energy resources (PERT)", "lang": "en"}, {"value": "Total erneuerbare Primärenergie (PERT)", "lang": "de"}], "type": "flow data set", "refObjectId": "53f97275-fa8a-4cdd-9024-65936002acd0", "uri": "../flows/53f97275-fa8a-4cdd-9024-65936002acd0.xml"}, "exchange direction": "INPUT", "other": {"anies": [{"name": "referenceToUnitGroupDataSet", "value": {"shortDescription": [{"value": "MJ", "lang": "en"}], "type": "unit group data set", "refObjectId": "93a60a57-a3c8-11da-a746-0800200c9a66", "uri": "../unitgroups/93a60a57-a3c8-11da-a746-0800200c9a66.xml"}}, {"value": "14378.6119090954", "module": "A1-A3"}, {"value": "0", "module": "C1"}, {"value": "0.573290680639056", "module": "C2"}, {"value": "20.6691130066602", "module": "C3"}, {"value": "0", "module": "C4"}, {"value": "-1204.76069363582", "module": "D"}]}, "resolvedFlowVersion": "38.00.000", "flowProperties": [], "typeOfFlow": "Other flow", "classification": {"classHierarchy": "Quantities / Environmental quantities / EPD EN 15804 / LCI indicators", "name": "GaBiCategories"}}, {"dataSetInternalID": 4, "referenceToFlowDataSet": {"shortDescription": [{"value": "Non renewable primary energy as energy carrier (PENRE)", "lang": "en"}, {"value": "Nicht-erneuerbare Primärenergie als Energieträger (PENRE)", "lang": "de"}], "type": "flow data set", "refObjectId": "ac857178-2b45-46ec-892a-a9a4332f0372", "uri": "../flows/ac857178-2b45-46ec-892a-a9a4332f0372.xml"}, "exchange direction": "INPUT", "other": {"anies": [{"name": "referenceToUnitGroupDataSet", "value": {"shortDescription": [{"value": "MJ", "lang": "en"}], "type": "unit group data set", "refObjectId": "93a60a57-a3c8-11da-a746-0800200c9a66", "uri": "../unitgroups/93a60a57-a3c8-11da-a746-0800200c9a66.xml"}}, {"value": "4061.35899736787", "module": "A1-A3"}, {"value": "0", "module": "C1"}, {"value": "45.0760246442098", "module": "C2"}, {"value": "1922.64260342406", "module": "C3"}, {"value": "0", "module": "C4"}, {"value": "-14616.989135551", "module": "D"}]}, "resolvedFlowVersion": "38.00.000", "flowProperties": [], "typeOfFlow": "Other flow", "classification": {"classHierarchy": "Quantities", "name": "GaBiCategories"}}, {"dataSetInternalID": 5, "referenceToFlowDataSet": {"shortDescription": [{"value": "Non renewable primary energy as material utilization (PENRM)", "lang": "en"}, {"value": "Nicht-erneuerbare Primärenergie zur stofflichen Nutzung (PENRM)", "lang": "de"}], "type": "flow data set", "refObjectId": "1421caa0-679d-4bf4-b282-0eb850ccae27", "uri": "../flows/1421caa0-679d-4bf4-b282-0eb850ccae27.xml"}, "exchange direction": "INPUT", "other": {"anies": [{"name": "referenceToUnitGroupDataSet", "value": {"shortDescription": [{"value": "MJ", "lang": "en"}], "type": "unit group data set", "refObjectId": "93a60a57-a3c8-11da-a746-0800200c9a66", "uri": "../unitgroups/93a60a57-a3c8-11da-a746-0800200c9a66.xml"}}, {"value": "1748.73678684715", "module": "A1-A3"}, {"value": "0", "module": "C1"}, {"value": "0", "module": "C2"}, {"value": "-1728.1", "module": "C3"}, {"value": "0", "module": "C4"}, {"value": "0", "module": "D"}]}, "resolvedFlowVersion": "38.00.000", "flowProperties": [], "typeOfFlow": "Other flow", "classification": {"classHierarchy": "Quantities", "name": "GaBiCategories"}}, {"dataSetInternalID": 6, "referenceToFlowDataSet": {"shortDescription": [{"value": "Total use of non renewable primary energy resources (PENRT)", "lang": "en"}, {"value": "Total nicht erneuerbare Primärenergie (PENRT)", "lang": "de"}], "type": "flow data set", "refObjectId": "06159210-646b-4c8d-8583-da9b3b95a6c1", "uri": "../flows/06159210-646b-4c8d-8583-da9b3b95a6c1.xml"}, "exchange direction": "INPUT", "other": {"anies": [{"name": "referenceToUnitGroupDataSet", "value": {"shortDescription": [{"value": "MJ", "lang": "en"}], "type": "unit group data set", "refObjectId": "93a60a57-a3c8-11da-a746-0800200c9a66", "uri": "../unitgroups/93a60a57-a3c8-11da-a746-0800200c9a66.xml"}}, {"value": "5810.09578421502", "module": "A1-A3"}, {"value": "0", "module": "C1"}, {"value": "45.0760246442098", "module": "C2"}, {"value": "194.542603424059", "module": "C3"}, {"value": "0", "module": "C4"}, {"value": "-14616.989135551", "module": "D"}]}, "resolvedFlowVersion": "38.00.000", "flowProperties": [], "typeOfFlow": "Other flow", "classification": {"classHierarchy": "Quantities / Environmental quantities / EPD EN 15804 / LCI indicators", "name": "GaBiCategories"}}, {"dataSetInternalID": 7, "referenceToFlowDataSet": {"shortDescription": [{"value": "Use of secondary material (SM)", "lang": "en"}, {"value": "Einsatz von Sekundärstoffen (SM)", "lang": "de"}], "type": "flow data set", "refObjectId": "c6a1f35f-2d09-4f54-8dfb-97e502e1ce92", "uri": "../flows/c6a1f35f-2d09-4f54-8dfb-97e502e1ce92.xml"}, "exchange direction": "INPUT", "other": {"anies": [{"name": "referenceToUnitGroupDataSet", "value": {"shortDescription": [{"value": "kg", "lang": "en"}], "type": "unit group data set", "refObjectId": "ad38d542-3fe9-439d-9b95-2f5f7752acaf", "uri": "../unitgroups/ad38d542-3fe9-439d-9b95-2f5f7752acaf.xml"}}, {"value": "0.00394170409220816", "module": "A1-A3"}, {"value": "0", "module": "C1"}, {"value": "0", "module": "C2"}, {"value": "0", "module": "C3"}, {"value": "0", "module": "C4"}, {"value": "0", "module": "D"}]}, "resolvedFlowVersion": "38.00.000", "flowProperties": [], "typeOfFlow": "Other flow", "classification": {"classHierarchy": "Quantities / Environmental quantities / EPD EN 15804 / LCI indicators", "name": "GaBiCategories"}}, {"dataSetInternalID": 8, "referenceToFlowDataSet": {"shortDescription": [{"value": "Use of renewable secondary fuels (RSF)", "lang": "en"}, {"value": "Erneuerbare Sekundärbrennstoffe (RSF)", "lang": "de"}], "type": "flow data set", "refObjectId": "64333088-a55f-4aa2-9a31-c10b07816787", "uri": "../flows/64333088-a55f-4aa2-9a31-c10b07816787.xml"}, "exchange direction": "INPUT", "other": {"anies": [{"name": "referenceToUnitGroupDataSet", "value": {"shortDescription": [{"value": "MJ", "lang": "en"}], "type": "unit group data set", "refObjectId": "93a60a57-a3c8-11da-a746-0800200c9a66", "uri": "../unitgroups/93a60a57-a3c8-11da-a746-0800200c9a66.xml"}}, {"value": "438.531366791244", "module": "A1-A3"}, {"value": "0", "module": "C1"}, {"value": "0", "module": "C2"}, {"value": "0", "module": "C3"}, {"value": "0", "module": "C4"}, {"value": "7848.27", "module": "D"}]}, "resolvedFlowVersion": "38.00.000", "flowProperties": [], "typeOfFlow": "Other flow", "classification": {"classHierarchy": "Quantities / Environmental quantities / EPD EN 15804 / LCI indicators", "name": "GaBiCategories"}}, {"dataSetInternalID": 9, "referenceToFlowDataSet": {"shortDescription": [{"value": "Use of non renewable secondary fuels (NRSF)", "lang": "en"}, {"value": "Nicht erneuerbare Sekundärbrennstoffe (NRSF)", "lang": "de"}], "type": "flow data set", "refObjectId": "89def144-d39a-4287-b86f-efde453ddcb2", "uri": "../flows/89def144-d39a-4287-b86f-efde453ddcb2.xml"}, "exchange direction": "INPUT", "other": {"anies": [{"name": "referenceToUnitGroupDataSet", "value": {"shortDescription": [{"value": "MJ", "lang": "en"}], "type": "unit group data set", "refObjectId": "93a60a57-a3c8-11da-a746-0800200c9a66", "uri": "../unitgroups/93a60a57-a3c8-11da-a746-0800200c9a66.xml"}}, {"value": "0", "module": "A1-A3"}, {"value": "0", "module": "C1"}, {"value": "0", "module": "C2"}, {"value": "0", "module": "C3"}, {"value": "0", "module": "C4"}, {"value": "1402.03", "module": "D"}]}, "resolvedFlowVersion": "38.00.000", "flowProperties": [], "typeOfFlow": "Other flow", "classification": {"classHierarchy": "Quantities / Environmental quantities / EPD EN 15804 / LCI indicators", "name": "GaBiCategories"}}, {"dataSetInternalID": 10, "referenceToFlowDataSet": {"shortDescription": [{"value": "Use of net fresh water (FW)", "lang": "en"}, {"value": "Einsatz von Süßwasserressourcen (FW)", "lang": "de"}], "type": "flow data set", "refObjectId": "3cf952c8-f3a4-461d-8c96-96456ca62246", "uri": "../flows/3cf952c8-f3a4-461d-8c96-96456ca62246.xml"}, "exchange direction": "INPUT", "other": {"anies": [{"name": "referenceToUnitGroupDataSet", "value": {"shortDescription": [{"value": "m^3", "lang": "en"}], "type": "unit group data set", "refObjectId": "cd950537-0a98-4044-9ba7-9f9a68d0a504", "uri": "../unitgroups/cd950537-0a98-4044-9ba7-9f9a68d0a504.xml"}}, {"value": "6.70322343300172", "module": "A1-A3"}, {"value": "0", "module": "C1"}, {"value": "0.00535809213265034", "module": "C2"}, {"value": "0.108424541668535", "module": "C3"}, {"value": "0", "module": "C4"}, {"value": "-5.8998615247528", "module": "D"}]}, "resolvedFlowVersion": "38.00.000", "flowProperties": [], "typeOfFlow": "Other flow", "classification": {"classHierarchy": "Quantities / Environmental quantities / EPD EN 15804 / LCI indicators", "name": "GaBiCategories"}}, {"dataSetInternalID": 11, "referenceToFlowDataSet": {"shortDescription": [{"value": "Hazardous waste disposed (HWD)", "lang": "en"}, {"value": "Gefährlicher Abfall zur Deponie (HWD)", "lang": "de"}], "type": "flow data set", "refObjectId": "430f9e0f-59b2-46a0-8e0d-55e0e84948fc", "uri": "../flows/430f9e0f-59b2-46a0-8e0d-55e0e84948fc.xml"}, "exchange direction": "OUTPUT", "other": {"anies": [{"name": "referenceToUnitGroupDataSet", "value": {"shortDescription": [{"value": "kg", "lang": "en"}], "type": "unit group data set", "refObjectId": "ad38d542-3fe9-439d-9b95-2f5f7752acaf", "uri": "../unitgroups/ad38d542-3fe9-439d-9b95-2f5f7752acaf.xml"}}, {"value": "9.89828650842322", "module": "A1-A3"}, {"value": "0", "module": "C1"}, {"value": "0.031183571991059", "module": "C2"}, {"value": "0.29007375427354", "module": "C3"}, {"value": "0", "module": "C4"}, {"value": "-2.2473626147426", "module": "D"}]}, "resolvedFlowVersion": "38.00.000", "flowProperties": [], "typeOfFlow": "Other flow", "classification": {"classHierarchy": "Quantities / Environmental quantities / EPD EN 15804 / LCI indicators", "name": "GaBiCategories"}}, {"dataSetInternalID": 12, "referenceToFlowDataSet": {"shortDescription": [{"value": "Non hazardous waste disposed (NHWD)", "lang": "en"}, {"value": "Entsorgter nicht gefährlicher Abfall (NHWD)", "lang": "de"}], "type": "flow data set", "refObjectId": "b29ef66b-e286-4afa-949f-62f1a7b4d7fa", "uri": "../flows/b29ef66b-e286-4afa-949f-62f1a7b4d7fa.xml"}, "exchange direction": "OUTPUT", "other": {"anies": [{"name": "referenceToUnitGroupDataSet", "value": {"shortDescription": [{"value": "kg", "lang": "en"}], "type": "unit group data set", "refObjectId": "ad38d542-3fe9-439d-9b95-2f5f7752acaf", "uri": "../unitgroups/ad38d542-3fe9-439d-9b95-2f5f7752acaf.xml"}}, {"value": "98.5984354737432", "module": "A1-A3"}, {"value": "0", "module": "C1"}, {"value": "4.44298645431486", "module": "C2"}, {"value": "7.9681433472043", "module": "C3"}, {"value": "0", "module": "C4"}, {"value": "-88.6452798356231", "module": "D"}]}, "resolvedFlowVersion": "38.00.000", "flowProperties": [], "typeOfFlow": "Other flow", "classification": {"classHierarchy": "Quantities / Environmental quantities / EPD EN 15804 / LCI indicators", "name": "GaBiCategories"}}, {"dataSetInternalID": 13, "referenceToFlowDataSet": {"shortDescription": [{"value": "Radioactive waste disposed (RWD)", "lang": "en"}, {"value": "Entsorgter radioaktiver Abfall (RWD)", "lang": "de"}], "type": "flow data set", "refObjectId": "3449546e-52ad-4b39-b809-9fb77cea8ff6", "uri": "../flows/3449546e-52ad-4b39-b809-9fb77cea8ff6.xml"}, "exchange direction": "OUTPUT", "other": {"anies": [{"name": "referenceToUnitGroupDataSet", "value": {"shortDescription": [{"value": "kg", "lang": "en"}], "type": "unit group data set", "refObjectId": "ad38d542-3fe9-439d-9b95-2f5f7752acaf", "uri": "../unitgroups/ad38d542-3fe9-439d-9b95-2f5f7752acaf.xml"}}, {"value": "0.0387202365644934", "module": "A1-A3"}, {"value": "0", "module": "C1"}, {"value": "0.000305178739020951", "module": "C2"}, {"value": "0.00135958553724948", "module": "C3"}, {"value": "0", "module": "C4"}, {"value": "-0.0580278815130109", "module": "D"}]}, "resolvedFlowVersion": "38.00.000", "flowProperties": [], "typeOfFlow": "Other flow", "classification": {"classHierarchy": "Quantities / Environmental quantities / EPD EN 15804 / LCI indicators", "name": "GaBiCategories"}}, {"dataSetInternalID": 14, "referenceToFlowDataSet": {"shortDescription": [{"value": "Components for re-use (CRU)", "lang": "en"}, {"value": "Komponenten für die Wiederverwendung (CRU)", "lang": "de"}], "type": "flow data set", "refObjectId": "a2b32f97-3fc7-4af2-b209-525bc6426f33", "uri": "../flows/a2b32f97-3fc7-4af2-b209-525bc6426f33.xml"}, "exchange direction": "OUTPUT", "other": {"anies": [{"name": "referenceToUnitGroupDataSet", "value": {"shortDescription": [{"value": "kg", "lang": "en"}], "type": "unit group data set", "refObjectId": "ad38d542-3fe9-439d-9b95-2f5f7752acaf", "uri": "../unitgroups/ad38d542-3fe9-439d-9b95-2f5f7752acaf.xml"}}, {"value": "0", "module": "A1-A3"}, {"value": "0", "module": "C1"}, {"value": "0", "module": "C2"}, {"value": "0", "module": "C3"}, {"value": "0", "module": "C4"}, {"value": "0", "module": "D"}]}, "resolvedFlowVersion": "38.00.000", "flowProperties": [], "typeOfFlow": "Other flow", "classification": {"classHierarchy": "Quantities / Environmental quantities / EPD EN 15804 / LCI indicators", "name": "GaBiCategories"}}, {"dataSetInternalID": 15, "referenceToFlowDataSet": {"shortDescription": [{"value": "Materials for recycling (MFR)", "lang": "en"}, {"value": "Stoffe zum Recycling (MFR)", "lang": "de"}], "type": "flow data set", "refObjectId": "d7fe48a5-4103-49c8-9aae-b0b5dfdbd6ae", "uri": "../flows/d7fe48a5-4103-49c8-9aae-b0b5dfdbd6ae.xml"}, "exchange direction": "OUTPUT", "other": {"anies": [{"name": "referenceToUnitGroupDataSet", "value": {"shortDescription": [{"value": "kg", "lang": "en"}], "type": "unit group data set", "refObjectId": "ad38d542-3fe9-439d-9b95-2f5f7752acaf", "uri": "../unitgroups/ad38d542-3fe9-439d-9b95-2f5f7752acaf.xml"}}, {"value": "0", "module": "A1-A3"}, {"value": "0", "module": "C1"}, {"value": "0", "module": "C2"}, {"value": "0", "module": "C3"}, {"value": "0", "module": "C4"}, {"value": "0", "module": "D"}]}, "resolvedFlowVersion": "38.00.000", "flowProperties": [], "typeOfFlow": "Other flow", "classification": {"classHierarchy": "Quantities / Environmental quantities / EPD EN 15804 / LCI indicators", "name": "GaBiCategories"}}, {"dataSetInternalID": 16, "referenceToFlowDataSet": {"shortDescription": [{"value": "Materials for energy recovery (MER)", "lang": "en"}, {"value": "Stoffe für die Energierückgewinnung (MER)", "lang": "de"}], "type": "flow data set", "refObjectId": "59a9181c-3aaf-46ee-8b13-2b3723b6e447", "uri": "../flows/59a9181c-3aaf-46ee-8b13-2b3723b6e447.xml"}, "exchange direction": "OUTPUT", "other": {"anies": [{"name": "referenceToUnitGroupDataSet", "value": {"shortDescription": [{"value": "kg", "lang": "en"}], "type": "unit group data set", "refObjectId": "ad38d542-3fe9-439d-9b95-2f5f7752acaf", "uri": "../unitgroups/ad38d542-3fe9-439d-9b95-2f5f7752acaf.xml"}}, {"value": "0", "module": "A1-A3"}, {"value": "0", "module": "C1"}, {"value": "0", "module": "C2"}, {"value": "636.82", "module": "C3"}, {"value": "0", "module": "C4"}, {"value": "0", "module": "D"}]}, "resolvedFlowVersion": "38.00.000", "flowProperties": [], "typeOfFlow": "Other flow", "classification": {"classHierarchy": "Quantities / Environmental quantities / EPD EN 15804 / LCI indicators", "name": "GaBiCategories"}}, {"dataSetInternalID": 17, "referenceToFlowDataSet": {"shortDescription": [{"value": "Exported electrical energy (EEE)", "lang": "en"}, {"value": "Exportierte elektrische Energie (EEE)", "lang": "de"}], "type": "flow data set", "refObjectId": "4da0c987-2b76-40d6-9e9e-82a017aaaf29", "uri": "../flows/4da0c987-2b76-40d6-9e9e-82a017aaaf29.xml"}, "exchange direction": "OUTPUT", "other": {"anies": [{"name": "referenceToUnitGroupDataSet", "value": {"shortDescription": [{"value": "MJ", "lang": "en"}], "type": "unit group data set", "refObjectId": "93a60a57-a3c8-11da-a746-0800200c9a66", "uri": "../unitgroups/93a60a57-a3c8-11da-a746-0800200c9a66.xml"}}, {"value": "0", "module": "A1-A3"}, {"value": "0", "module": "C1"}, {"value": "0", "module": "C2"}, {"value": "0", "module": "C3"}, {"value": "0", "module": "C4"}, {"value": "0", "module": "D"}]}, "resolvedFlowVersion": "38.00.000", "flowProperties": [], "typeOfFlow": "Other flow", "classification": {"classHierarchy": "Quantities / Environmental quantities / EPD EN 15804 / LCI indicators", "name": "GaBiCategories"}}, {"dataSetInternalID": 18, "referenceToFlowDataSet": {"shortDescription": [{"value": "Exported thermal energy (EET)", "lang": "en"}, {"value": "Exportierte thermische Energie (EET)", "lang": "de"}], "type": "flow data set", "refObjectId": "98daf38a-7a79-46d3-9a37-2b7bd0955810", "uri": "../flows/98daf38a-7a79-46d3-9a37-2b7bd0955810.xml"}, "exchange direction": "OUTPUT", "other": {"anies": [{"name": "referenceToUnitGroupDataSet", "value": {"shortDescription": [{"value": "MJ", "lang": "en"}], "type": "unit group data set", "refObjectId": "93a60a57-a3c8-11da-a746-0800200c9a66", "uri": "../unitgroups/93a60a57-a3c8-11da-a746-0800200c9a66.xml"}}, {"value": "0", "module": "A1-A3"}, {"value": "0", "module": "C1"}, {"value": "0", "module": "C2"}, {"value": "0", "module": "C3"}, {"value": "0", "module": "C4"}, {"value": "0", "module": "D"}]}, "resolvedFlowVersion": "38.00.000", "flowProperties": [], "typeOfFlow": "Other flow", "classification": {"classHierarchy": "Quantities / Environmental quantities / EPD EN 15804 / LCI indicators", "name": "GaBiCategories"}}]}, "LCIAResults": {"LCIAResult": [{"referenceToLCIAMethodDataSet": {"shortDescription": [{"value": "Global Warming Potential total (GWP-total)", "lang": "en"}, {"value": "Globales Erwärmungspotenzial total (GWP-total)", "lang": "de"}], "type": "LCIA method data set", "refObjectId": "6a37f984-a4b3-458a-a20a-64418c145fa2", "uri": "../lciamethods/6a37f984-a4b3-458a-a20a-64418c145fa2.xml"}, "other": {"anies": [{"name": "referenceToUnitGroupDataSet", "value": {"shortDescription": [{"value": "kg CO_(2) eq", "lang": "en"}], "type": "unit group data set", "refObjectId": "1ebf3012-d0db-4de2-aefd-ef30cedb0be1", "uri": "../unitgroups/1ebf3012-d0db-4de2-aefd-ef30cedb0be1.xml"}}, {"value": "-764.956228059906", "module": "A1-A3"}, {"value": "0", "module": "C1"}, {"value": "2.74802395950809", "module": "C2"}, {"value": "939.511526051137", "module": "C3"}, {"value": "0", "module": "C4"}, {"value": "-562.866673242946", "module": "D"}]}}, {"referenceToLCIAMethodDataSet": {"shortDescription": [{"value": "Global Warming Potential fossil fuels (GWP-fossil)", "lang": "en"}, {"value": "Globales Erwärmungspotenzial fossil (GWP-fossil)", "lang": "de"}], "type": "LCIA method data set", "refObjectId": "5f635281-343e-44fb-83df-1971b155e6b6", "uri": "../lciamethods/5f635281-343e-44fb-83df-1971b155e6b6.xml"}, "other": {"anies": [{"name": "referenceToUnitGroupDataSet", "value": {"shortDescription": [{"value": "kg CO_(2) eq", "lang": "en"}], "type": "unit group data set", "refObjectId": "1ebf3012-d0db-4de2-aefd-ef30cedb0be1", "uri": "../unitgroups/1ebf3012-d0db-4de2-aefd-ef30cedb0be1.xml"}}, {"value": "162.15371711887", "module": "A1-A3"}, {"value": "0", "module": "C1"}, {"value": "2.7460719656978", "module": "C2"}, {"value": "10.7486549326114", "module": "C3"}, {"value": "0", "module": "C4"}, {"value": "-560.908021286555", "module": "D"}]}}, {"referenceToLCIAMethodDataSet": {"shortDescription": [{"value": "Global Warming Potential biogenic (GWP-biogenic)", "lang": "en"}, {"value": "Globales Erwärmungspotenzial biogen (GWP-biogenic)", "lang": "de"}], "type": "LCIA method data set", "refObjectId": "2356e1ab-0185-4db5-86e5-16de51c7485c", "uri": "../lciamethods/2356e1ab-0185-4db5-86e5-16de51c7485c.xml"}, "other": {"anies": [{"name": "referenceToUnitGroupDataSet", "value": {"shortDescription": [{"value": "kg CO_(2) eq", "lang": "en"}], "type": "unit group data set", "refObjectId": "1ebf3012-d0db-4de2-aefd-ef30cedb0be1", "uri": "../unitgroups/1ebf3012-d0db-4de2-aefd-ef30cedb0be1.xml"}}, {"value": "-928.279400907472", "module": "A1-A3"}, {"value": "0", "module": "C1"}, {"value": "0.000891285800007091", "module": "C2"}, {"value": "928.748248162131", "module": "C3"}, {"value": "0", "module": "C4"}, {"value": "-1.11306011494979", "module": "D"}]}}, {"referenceToLCIAMethodDataSet": {"shortDescription": [{"value": "Global Warming Potential luluc (GWP-luluc)", "lang": "en"}, {"value": "Globales Erwärmungspotenzial luluc (GWP-luluc)", "lang": "de"}], "type": "LCIA method data set", "refObjectId": "4331bbdb-978a-490d-8707-eeb047f01a55", "uri": "../lciamethods/4331bbdb-978a-490d-8707-eeb047f01a55.xml"}, "other": {"anies": [{"name": "referenceToUnitGroupDataSet", "value": {"shortDescription": [{"value": "kg CO_(2) eq", "lang": "en"}], "type": "unit group data set", "refObjectId": "1ebf3012-d0db-4de2-aefd-ef30cedb0be1", "uri": "../unitgroups/1ebf3012-d0db-4de2-aefd-ef30cedb0be1.xml"}}, {"value": "1.16945572869253", "module": "A1-A3"}, {"value": "0", "module": "C1"}, {"value": "0.00106070801028882", "module": "C2"}, {"value": "0.0146229563947134", "module": "C3"}, {"value": "0", "module": "C4"}, {"value": "-0.845591841440965", "module": "D"}]}}, {"referenceToLCIAMethodDataSet": {"shortDescription": [{"value": "Depletion potential of the stratospheric ozone layer (ODP)", "lang": "en"}, {"value": "Abbau Potential der stratosphärischen Ozonschicht (ODP)", "lang": "de"}], "type": "LCIA method data set", "refObjectId": "b5c629d6-def3-11e6-bf01-fe55135034f3", "uri": "../lciamethods/b5c629d6-def3-11e6-bf01-fe55135034f3.xml"}, "other": {"anies": [{"name": "referenceToUnitGroupDataSet", "value": {"shortDescription": [{"value": "kg CFC11 eq", "lang": "en"}], "type": "unit group data set", "refObjectId": "d9e957c9-7309-4474-bf3a-7777df6c4e5b", "uri": "../unitgroups/d9e957c9-7309-4474-bf3a-7777df6c4e5b.xml"}}, {"value": "3.16324415437457E-05", "module": "A1-A3"}, {"value": "0", "module": "C1"}, {"value": "6.9068551578946E-07", "module": "C2"}, {"value": "1.54421302759544E-06", "module": "C3"}, {"value": "0", "module": "C4"}, {"value": "-7.92833638264874E-05", "module": "D"}]}}, {"referenceToLCIAMethodDataSet": {"shortDescription": [{"value": "Acidification potential of land and water (AP)", "lang": "en"}, {"value": "Versauerungspotenzial von Boden und Wasser (AP)", "lang": "de"}], "type": "LCIA method data set", "refObjectId": "b5c611c6-def3-11e6-bf01-fe55135034f3", "uri": "../lciamethods/b5c611c6-def3-11e6-bf01-fe55135034f3.xml"}, "other": {"anies": [{"name": "referenceToUnitGroupDataSet", "value": {"shortDescription": [{"value": "mol H^(+) eq", "lang": "en"}], "type": "unit group data set", "refObjectId": "42e089ac-92bf-4bf2-8ca1-5fc40d18f2ed", "uri": "../unitgroups/42e089ac-92bf-4bf2-8ca1-5fc40d18f2ed.xml"}}, {"value": "1.20372391150184", "module": "A1-A3"}, {"value": "0", "module": "C1"}, {"value": "0.00882255342950414", "module": "C2"}, {"value": "0.0605357368904144", "module": "C3"}, {"value": "0", "module": "C4"}, {"value": "-0.778109541267394", "module": "D"}]}}, {"referenceToLCIAMethodDataSet": {"shortDescription": [{"value": "Eutrophication potential aquatic freshwater (EP-freshwater)", "lang": "en"}, {"value": "Eutrophierungspotenzial Süßwasser (EP-freshwater)", "lang": "de"}], "type": "LCIA method data set", "refObjectId": "b53ec18f-7377-4ad3-86eb-cc3f4f276b2b", "uri": "../lciamethods/b53ec18f-7377-4ad3-86eb-cc3f4f276b2b.xml"}, "other": {"anies": [{"name": "referenceToUnitGroupDataSet", "value": {"shortDescription": [{"value": "kg P eq", "lang": "en"}], "type": "unit group data set", "refObjectId": "0429039d-a61d-4590-ba67-aa4a20a810a1", "uri": "../unitgroups/0429039d-a61d-4590-ba67-aa4a20a810a1.xml"}}, {"value": "0.0124455237084363", "module": "A1-A3"}, {"value": "0", "module": "C1"}, {"value": "1.97599773467376E-05", "module": "C2"}, {"value": "0.00059002329918623", "module": "C3"}, {"value": "0", "module": "C4"}, {"value": "-0.0371324994262385", "module": "D"}]}}, {"referenceToLCIAMethodDataSet": {"shortDescription": [{"value": "Eutrophication potential aquatic marine (EP-marine)", "lang": "en"}, {"value": "Eutrophierungspotenzial Salzwasser (EP-marine)", "lang": "de"}], "type": "LCIA method data set", "refObjectId": "b5c619fa-def3-11e6-bf01-fe55135034f3", "uri": "../lciamethods/b5c619fa-def3-11e6-bf01-fe55135034f3.xml"}, "other": {"anies": [{"name": "referenceToUnitGroupDataSet", "value": {"shortDescription": [{"value": "kg N eq", "lang": "en"}], "type": "unit group data set", "refObjectId": "d05bb823-ecdf-4686-8c40-bf1d9257859f", "uri": "../unitgroups/d05bb823-ecdf-4686-8c40-bf1d9257859f.xml"}}, {"value": "0.420682972250147", "module": "A1-A3"}, {"value": "0", "module": "C1"}, {"value": "0.00194067978397149", "module": "C2"}, {"value": "0.0154285619838929", "module": "C3"}, {"value": "0", "module": "C4"}, {"value": "0.380004637020928", "module": "D"}]}}, {"referenceToLCIAMethodDataSet": {"shortDescription": [{"value": "Eutrophication potential terrestrial (EP-terrestrial)", "lang": "en"}, {"value": "Eutrophierungspotenzial Land (EP-terrestrial)", "lang": "de"}], "type": "LCIA method data set", "refObjectId": "b5c614d2-def3-11e6-bf01-fe55135034f3", "uri": "../lciamethods/b5c614d2-def3-11e6-bf01-fe55135034f3.xml"}, "other": {"anies": [{"name": "referenceToUnitGroupDataSet", "value": {"shortDescription": [{"value": "mol N eq", "lang": "en"}], "type": "unit group data set", "refObjectId": "71b4d617-0ec9-4d3f-b65e-e438940c2401", "uri": "../unitgroups/71b4d617-0ec9-4d3f-b65e-e438940c2401.xml"}}, {"value": "3.96272445113776", "module": "A1-A3"}, {"value": "0", "module": "C1"}, {"value": "0.0215771983977636", "module": "C2"}, {"value": "0.172216033364323", "module": "C3"}, {"value": "0", "module": "C4"}, {"value": "4.11600860359455", "module": "D"}]}}, {"referenceToLCIAMethodDataSet": {"shortDescription": [{"value": "Formation potential of tropospheric ozone photochemical oxidants (POCP)", "lang": "en"}, {"value": "Bildungspotential für troposphärisches Ozon (POCP)", "lang": "de"}], "type": "LCIA method data set", "refObjectId": "b5c610fe-def3-11e6-bf01-fe55135034f3", "uri": "../lciamethods/b5c610fe-def3-11e6-bf01-fe55135034f3.xml"}, "other": {"anies": [{"name": "referenceToUnitGroupDataSet", "value": {"shortDescription": [{"value": "kg NMVOC eq", "lang": "en"}], "type": "unit group data set", "refObjectId": "d27c25f8-fbc1-44c6-b47b-4adbae4199c6", "uri": "../unitgroups/d27c25f8-fbc1-44c6-b47b-4adbae4199c6.xml"}}, {"value": "1.60340490191468", "module": "A1-A3"}, {"value": "0", "module": "C1"}, {"value": "0.0084969609039817", "module": "C2"}, {"value": "0.0488314794306688", "module": "C3"}, {"value": "0", "module": "C4"}, {"value": "0.743138012992945", "module": "D"}]}}, {"referenceToLCIAMethodDataSet": {"shortDescription": [{"value": "Abiotic depletion potential for non fossil resources (ADPE)", "lang": "en"}, {"value": "Potenzial für den abiotischen Abbau nicht fossiler Ressourcen (ADPE)", "lang": "de"}], "type": "LCIA method data set", "refObjectId": "b2ad6494-c78d-11e6-9d9d-cec0c932ce01", "uri": "../lciamethods/b2ad6494-c78d-11e6-9d9d-cec0c932ce01.xml"}, "other": {"anies": [{"name": "referenceToUnitGroupDataSet", "value": {"shortDescription": [{"value": "kg Sb eq", "lang": "en"}], "type": "unit group data set", "refObjectId": "54ccd2d9-a32a-4fc2-923d-f2c8c93e89d4", "uri": "../unitgroups/54ccd2d9-a32a-4fc2-923d-f2c8c93e89d4.xml"}}, {"value": "0.00207353319479529", "module": "A1-A3"}, {"value": "0", "module": "C1"}, {"value": "6.83783076208095E-06", "module": "C2"}, {"value": "3.57853897351397E-05", "module": "C3"}, {"value": "0", "module": "C4"}, {"value": "-0.000183751589186809", "module": "D"}]}}, {"referenceToLCIAMethodDataSet": {"shortDescription": [{"value": "Abiotic depletion potential for fossil resources (ADPF)", "lang": "en"}, {"value": "Potenzial für den abiotischen Abbau fossiler Brennstoffe (ADPF)", "lang": "de"}], "type": "LCIA method data set", "refObjectId": "b2ad6110-c78d-11e6-9d9d-cec0c932ce01", "uri": "../lciamethods/b2ad6110-c78d-11e6-9d9d-cec0c932ce01.xml"}, "other": {"anies": [{"name": "referenceToUnitGroupDataSet", "value": {"shortDescription": [{"value": "MJ", "lang": "en"}], "type": "unit group data set", "refObjectId": "93a60a57-a3c8-11da-a746-0800200c9a66", "uri": "../unitgroups/93a60a57-a3c8-11da-a746-0800200c9a66.xml"}}, {"value": "5817.958230984", "module": "A1-A3"}, {"value": "0", "module": "C1"}, {"value": "45.0738933366912", "module": "C2"}, {"value": "194.536028947111", "module": "C3"}, {"value": "0", "module": "C4"}, {"value": "-14616.925740627", "module": "D"}]}}, {"referenceToLCIAMethodDataSet": {"shortDescription": [{"value": "Water use (WDP)", "lang": "en"}, {"value": "Wassernutzung (WDP)", "lang": "de"}], "type": "LCIA method data set", "refObjectId": "b2ad66ce-c78d-11e6-9d9d-cec0c932ce01", "uri": "../lciamethods/b2ad66ce-c78d-11e6-9d9d-cec0c932ce01.xml"}, "other": {"anies": [{"name": "referenceToUnitGroupDataSet", "value": {"shortDescription": [{"value": "m^(3) world eq deprived", "lang": "en"}], "type": "unit group data set", "refObjectId": "6ae2df01-888e-46c8-b17d-49fa3869b476", "uri": "../unitgroups/6ae2df01-888e-46c8-b17d-49fa3869b476.xml"}}, {"value": "229.802530773589", "module": "A1-A3"}, {"value": "0", "module": "C1"}, {"value": "0.152357432349657", "module": "C2"}, {"value": "0.540858013315984", "module": "C3"}, {"value": "0", "module": "C4"}, {"value": "-79.9014558186135", "module": "D"}]}}, {"referenceToLCIAMethodDataSet": {"shortDescription": [{"value": "Incidence of disease due to PM emissions (PM)", "lang": "en"}, {"value": "Auftreten von Krankheiten aufgrund von Feinstaubemissionen (PM)", "lang": "de"}], "type": "LCIA method data set", "refObjectId": "b5c602c6-def3-11e6-bf01-fe55135034f3", "uri": "../lciamethods/b5c602c6-def3-11e6-bf01-fe55135034f3.xml"}, "other": {"anies": [{"name": "referenceToUnitGroupDataSet", "value": {"shortDescription": [{"value": "Disease incidence", "lang": "en"}], "type": "unit group data set", "refObjectId": "3883559b-648f-4afc-8ba2-0bd24f3affa3", "uri": "../unitgroups/3883559b-648f-4afc-8ba2-0bd24f3affa3.xml"}}, {"value": "9.54554245175151E-06", "module": "A1-A3"}, {"value": "0", "module": "C1"}, {"value": "3.214110002903E-07", "module": "C2"}, {"value": "7.12896587648579E-07", "module": "C3"}, {"value": "0", "module": "C4"}, {"value": "8.11626379830589E-06", "module": "D"}]}}, {"referenceToLCIAMethodDataSet": {"shortDescription": [{"value": "Human exposure efficiency relative to U235 (IR)", "lang": "en"}, {"value": "Wirkung durch Exposition des Menschen mit U235 (IR)", "lang": "de"}], "type": "LCIA method data set", "refObjectId": "b5c632be-def3-11e6-bf01-fe55135034f3", "uri": "../lciamethods/b5c632be-def3-11e6-bf01-fe55135034f3.xml"}, "other": {"anies": [{"name": "referenceToUnitGroupDataSet", "value": {"shortDescription": [{"value": "kBq U235 eq", "lang": "en"}], "type": "unit group data set", "refObjectId": "456b05bf-1415-44a9-9993-02452f554c09", "uri": "../unitgroups/456b05bf-1415-44a9-9993-02452f554c09.xml"}}, {"value": "30.0994343254878", "module": "A1-A3"}, {"value": "0", "module": "C1"}, {"value": "0.195474658639722", "module": "C2"}, {"value": "1.33173226008384", "module": "C3"}, {"value": "0", "module": "C4"}, {"value": "-66.8009953177125", "module": "D"}]}}, {"referenceToLCIAMethodDataSet": {"shortDescription": [{"value": "Comparative toxic unit for ecosystems (ETP-fw)", "lang": "en"}, {"value": "Toxizitätsvergleichseinheit für Ökosysteme (ETP-fw)", "lang": "de"}], "type": "LCIA method data set", "refObjectId": "ee1082d1-b0f7-43ca-a1f0-21e2a4a74511", "uri": "../lciamethods/ee1082d1-b0f7-43ca-a1f0-21e2a4a74511.xml"}, "other": {"anies": [{"name": "referenceToUnitGroupDataSet", "value": {"shortDescription": [{"value": "CTUe", "lang": "en"}], "type": "unit group data set", "refObjectId": "aa959ded-f1eb-4efb-9c5c-2d60be36b3e6", "uri": "../unitgroups/aa959ded-f1eb-4efb-9c5c-2d60be36b3e6.xml"}}, {"value": "0.000128579332679927", "module": "A1-A3"}, {"value": "0", "module": "C1"}, {"value": "5.51648937577091E-08", "module": "C2"}, {"value": "2.71016963810887E-07", "module": "C3"}, {"value": "0", "module": "C4"}, {"value": "-1.47617899412453E-06", "module": "D"}]}}, {"referenceToLCIAMethodDataSet": {"shortDescription": [{"value": "Comparative toxic unit for humans (carcinogenic) (HTP-c)", "lang": "en"}, {"value": "Toxizitätsvergleichseinheit für Menschen (krebserregend) (HTP-c)", "lang": "de"}], "type": "LCIA method data set", "refObjectId": "2299222a-bbd8-474f-9d4f-4dd1f18aea7c", "uri": "../lciamethods/2299222a-bbd8-474f-9d4f-4dd1f18aea7c.xml"}, "other": {"anies": [{"name": "referenceToUnitGroupDataSet", "value": {"shortDescription": [{"value": "CTUh", "lang": "en"}], "type": "unit group data set", "refObjectId": "d4c9523e-2d7e-49fd-8469-998f547d3a70", "uri": "../unitgroups/d4c9523e-2d7e-49fd-8469-998f547d3a70.xml"}}, {"value": "9.90413585081848E-07", "module": "A1-A3"}, {"value": "0", "module": "C1"}, {"value": "4.48122026901457E-10", "module": "C2"}, {"value": "3.01520056120865E-09", "module": "C3"}, {"value": "0", "module": "C4"}, {"value": "3.20235939937953E-08", "module": "D"}]}}, {"referenceToLCIAMethodDataSet": {"shortDescription": [{"value": "Comparative toxic unit for humans (noncarcinogenic) (HTP-nc)", "lang": "en"}, {"value": "Toxizitätsvergleichseinheit für Menschen (nicht krebserregend) (HTP-nc)", "lang": "de"}], "type": "LCIA method data set", "refObjectId": "3af763a5-b7a1-48c9-9cee-1f223481fcef", "uri": "../lciamethods/3af763a5-b7a1-48c9-9cee-1f223481fcef.xml"}, "other": {"anies": [{"name": "referenceToUnitGroupDataSet", "value": {"shortDescription": [{"value": "CTUh", "lang": "en"}], "type": "unit group data set", "refObjectId": "d4c9523e-2d7e-49fd-8469-998f547d3a70", "uri": "../unitgroups/d4c9523e-2d7e-49fd-8469-998f547d3a70.xml"}}, {"value": "1.38833442648164E-07", "module": "A1-A3"}, {"value": "0", "module": "C1"}, {"value": "1.25049250886681E-09", "module": "C2"}, {"value": "9.93359474730182E-09", "module": "C3"}, {"value": "0", "module": "C4"}, {"value": "-6.72339585813507E-08", "module": "D"}]}}, {"referenceToLCIAMethodDataSet": {"shortDescription": [{"value": "Soil quality index (SQP)", "lang": "en"}, {"value": "Bodenqualitätsindex (SQP)", "lang": "de"}], "type": "LCIA method data set", "refObjectId": "b2ad6890-c78d-11e6-9d9d-cec0c932ce01", "uri": "../lciamethods/b2ad6890-c78d-11e6-9d9d-cec0c932ce01.xml"}, "other": {"anies": [{"name": "referenceToUnitGroupDataSet", "value": {"shortDescription": [{"value": "SQP", "lang": "en"}], "type": "unit group data set", "refObjectId": "f130951c-e67f-4f7f-8dd4-665de3974e18", "uri": "../unitgroups/f130951c-e67f-4f7f-8dd4-665de3974e18.xml"}}, {"value": "59566.7514766916", "module": "A1-A3"}, {"value": "0", "module": "C1"}, {"value": "51.5480015029526", "module": "C2"}, {"value": "94.7918841735863", "module": "C3"}, {"value": "0", "module": "C4"}, {"value": "-1140.97956056738", "module": "D"}]}}]}, "otherAttributes": {"{http://www.indata.network/EPD/2019}epd-version": "1.2"}, "version": "1.1", "locations": "../ILCDLocations.xml"}