{"processInformation": {"dataSetInformation": {"UUID": "22cfb204-8185-499c-b764-e53cd419bcca", "name": {"baseName": [{"value": "Window operator for VELUX GGL/GGU (KMG 100K) and control system (KUX 110), mains connected", "lang": "en"}, {"value": "Fensterantrieb für VELUX GGL/GGU (KMG 100K) und kontrollsystem (KUX 110), grid", "lang": "de"}], "functionalUnitFlowProperties": [{"lang": "en"}]}, "classificationInformation": {"classification": [{"class": [{"value": "Komponenten von Fenstern und Vorhangfassaden", "level": 0, "classId": "7"}, {"value": "Antriebssysteme", "level": 1, "classId": "7.7"}, {"value": "elektrisch", "level": 2, "classId": "7.7.02"}], "name": "OEKOBAU.DAT"}, {"class": [{"value": "02 Building products", "level": 0}, {"value": "Doors, windows, shutters, and related products", "level": 1}, {"value": "Drive systems for automatic doors and gates", "level": 2}], "name": "IBUCategories"}]}, "generalComment": [{"value": "EPD covering VELUX electrical window operator for the mains connected window type VELUX INTEGRA GGL/GGU. The operator consists of a chain operator, a rain sensor, a control system and a remote. The products are manufactured by the VELUX Group at a production site in the Czech Republic.", "lang": "en"}, {"value": "Der Antrieb besteht aus einem Kettenantrieb, einem Regensensor, einem Steuerungssystem und einer Fernbedienung.", "lang": "de"}]}, "quantitativeReference": {"referenceToReferenceFlow": [0]}, "time": {"referenceYear": 2023, "dataSetValidUntil": 2028, "other": {"anies": [{"name": "publicationDateOfEPD", "value": 1683763200000}]}}, "geography": {"locationOfOperationSupplyOrProduction": {"location": "RER"}}, "technology": {"technologyDescriptionAndIncludedProcesses": [{"value": "The VELUX INTEGRA GGL/GPL window operators are a mains connected ventilation system. They are made up of a chain operator, a control system, a rain sensor and a remote. The products are assembled at a VELUX production site and are either integrated with new windows or sold separately for retrofitting. \nTechnical data: \nThe CE marking for electrical window operators does not specify the need for a Declaration of Performance. Instead, a Declaration of Conformity is required.\nThe performance values relevant for the product are specified in the table below. \nDeclared unit: \nThe declared unit is one piece. This corresponds to an electrical window operator system, including a chain operator, a control system, a rain sensor and a remote.", "lang": "en"}, {"value": "Die VELUX INTEGRA GGL/GPL Fensterantriebe sind ein netzgebundenes Lüftungssystem. Sie bestehen aus einem Kettenantrieb, einem Steuerungssystem, einem Regensensor und einer Fernbedienung. Die Produkte werden in einer VELUX Produktionsstätte zusammengebaut und entweder in neue Fenster integriert oder separat zum Nachrüsten verkauft. \nTechnische Daten: \nDie CE-Kennzeichnung für elektrische Fensterantriebe schreibt keine Leistungserklärung vor. Stattdessen ist eine Konformitätserklärung erforderlich. \nDeklarierte Einheit: \n1 stück", "lang": "de"}], "technologicalApplicability": [{"value": "The VELUX electrical window operator is sold separately for retrofitting.", "lang": "en"}, {"value": "Der elektrische Fensterantrieb von VELUX ist separat erhältlich und kann nachgerüstet werden.", "lang": "de"}]}}, "modellingAndValidation": {"LCIMethodAndAllocation": {"typeOfDataSet": "EPD", "referenceToLCAMethodDetails": [{"shortDescription": [{"value": "Drive systems for automatic doors and gates.pdf", "lang": "en"}], "type": "source data set", "refObjectId": "963d27a9-03e1-4bf9-be8f-684819bad792"}], "other": {"anies": [{"name": "subType", "value": "average dataset"}]}}, "dataSourcesTreatmentAndRepresentativeness": {"referenceToDataSource": [{"shortDescription": [{"value": "GaBi Database (all versions)", "lang": "en"}], "type": "source data set", "refObjectId": "28d74cc0-db8b-4d7e-bc44-5f6d56ce0c4a"}, {"shortDescription": [{"value": "GaBi Database Edition 2021, CUP 2021.02", "lang": "en"}], "type": "source data set", "refObjectId": "90321ffe-9ebb-4946-886c-338efe6fbf26"}], "useAdviceForDataSet": [{"value": "Scope: \nThe EPD is a specific EPD covering VELUX electrical window operator for the mains connected window type VELUX INTEGRA GGL/GGU. The operator consists of a chain operator, a rain sensor, a control system and a remote. The products are manufactured by the VELUX Group at a production site in the Czech Republic. \nSystem boundary: \nType of EPD:\nCradle to gate - with options. The following life cycle phases were considered:\n\nProduct stage:\n\nA1 - Raw material supply: extraction and processing, production of the pre-products (e.g. motor suspension, PCB, battery...). Production of packaging: cardboard boxes, paper labels, EPS and plastic film. \n\nA2 - Transport: Transport of pre-products and packaging components to the manufacturing sites.\n\nA3 - Manufacturing: The products are produced/assembled at the VELUX production site, where the finished window operator is ready for shipment.\n\nEnd of life stage: \n\nC1 - De-construction/demolition: de-construction of the product with the use of manual hand tools.\n\nC2 - Transport: transport of the product to waste treatment including to and from sorting and shredding facilities.\n\nC3 - Waste processing: includes sorting, shredding, incineration and recycling processes. \n\nC4 - Disposal: disposal of all materials\n\nBenefits and loads beyond the system boundaries:\n\nD - Reuse, recovery and recycling potential: benefits from plastic incineration processes and material recycling. End of life includes all activities from when the product reaches the end of its service life and no longer provides any functionality until all materials and components are processed for reuse/recycling/energy recovery or are disposed of.\n\nThe applied end-of-life scenario follows the requirements in the PCR Part A, chapter 6.2 regarding complex products, with a combination of recycling, thermal waste treatment and landfilling. 100% of the material is considered in the end-of-life scenario. Generally metals, cables, batteries and polychlorinated biphenyl (PCB)'s are recycled, plastic parts are incinerated with energy recovery and magnets are landfilled.", "lang": "en"}, {"value": "Gültigkeitsbereich: \nDie EPD ist spezuifisch und inkludiert ein stück elektrische Fensterantriebe verkauft in Europa \nSystemgrenze: \nCradle to gate - mit Optionen: inkludiert die Module A1, A2, A3, C1, C2, C3, C4 und D.", "lang": "de"}], "other": {"anies": [{"name": "referenceToOriginalEPD", "value": {"shortDescription": {"value": "Window operator for VELUX GGL/GGU (KMG 100K) and control system (KUX 110), mains connected.pdf", "defaultValue": "Window operator for VELUX GGL/GGU (KMG 100K) and control system (KUX 110), mains connected.pdf", "lstrings": [{"lang": "en", "value": "Window operator for VELUX GGL/GGU (KMG 100K) and control system (KUX 110), mains connected.pdf"}]}, "type": "source data set", "uuid": {"uuid": "d067d387-3ae2-477b-a481-b8c1e9da49c6"}, "refObjectId": "d067d387-3ae2-477b-a481-b8c1e9da49c6", "resourceURLs": ["https://oekobaudat.de/OEKOBAU.DAT/resource/sources/d067d387-3ae2-477b-a481-b8c1e9da49c6/Window_operator_for_VELUX_pivot_hinged_windows_KMG_100K_and_control_system_KUX_110_mains_connected_20694.pdf?version=00.03.000"]}}]}}, "validation": {"review": [{"referenceToNameOfReviewerAndInstitution": [{"shortDescription": [{"value": "Institut Bauen und Umwelt e. V.", "lang": "en"}], "type": "contact data set", "refObjectId": "d111dbec-b024-4be5-86c5-752d6eb2cf95", "uri": "../contacts/d111dbec-b024-4be5-86c5-752d6eb2cf95.xml"}], "type": "Accredited third party review"}]}, "complianceDeclarations": {"compliance": [{"referenceToComplianceSystem": {"shortDescription": [{"value": "DIN EN 15804+A2", "lang": "en"}], "type": "source data set", "refObjectId": "c0016b33-8cf7-415c-ac6e-deba0d21440d", "uri": "../sources/c0016b33-8cf7-415c-ac6e-deba0d21440d.xml"}}, {"referenceToComplianceSystem": {"shortDescription": [{"value": "ISO 14025", "lang": "en"}], "type": "source data set", "refObjectId": "4f2eb655-6e44-4874-a95a-e28f5442cd4d", "uri": "../sources/4f2eb655-6e44-4874-a95a-e28f5442cd4d.xml"}}]}}, "administrativeInformation": {"commissionerAndGoal": {"referenceToCommissioner": [{"shortDescription": [{"value": "VELUX Group", "lang": "en"}], "type": "contact data set", "refObjectId": "ab62e83b-7504-48ae-abdc-def53c14790d", "uri": "../contacts/ab62e83b-7504-48ae-abdc-def53c14790d.xml"}]}, "dataGenerator": {"referenceToPersonOrEntityGeneratingTheDataSet": [{"shortDescription": [{"value": "FORCE Technology", "lang": "en"}], "type": "contact data set", "refObjectId": "827dee6d-fd7f-4856-a4e8-0b3be8abfe6c", "uri": "../contacts/827dee6d-fd7f-4856-a4e8-0b3be8abfe6c.xml"}]}, "dataEntryBy": {"timeStamp": 1683763200000, "referenceToDataSetFormat": [{"shortDescription": [{"value": "ILCD Format", "lang": "en"}], "type": "source data set", "refObjectId": "a97a0155-0234-4b87-b4ce-a45da52f2a40", "uri": "../sources/a97a0155-0234-4b87-b4ce-a45da52f2a40.xml"}, {"shortDescription": [{"value": "EPD-Datenformaterweiterungen v1.2", "lang": "de"}, {"value": "EPD Data Format Extensions v1.2", "lang": "en"}], "type": "source data set", "refObjectId": "a29449fd-aa2f-4de8-b5d7-4b06b43c6fde", "uri": "../sources/a29449fd-aa2f-4de8-b5d7-4b06b43c6fde.xml"}]}, "publicationAndOwnership": {"dataSetVersion": "00.03.000", "referenceToRegistrationAuthority": {"shortDescription": [{"value": "Institut Bauen und Umwelt e. V.", "lang": "en"}], "type": "contact data set", "refObjectId": "d111dbec-b024-4be5-86c5-752d6eb2cf95", "uri": "../contacts/d111dbec-b024-4be5-86c5-752d6eb2cf95.xml"}, "registrationNumber": "EPD-VEL-20230051-IBA1-EN", "referenceToOwnershipOfDataSet": {"shortDescription": [{"value": "VELUX Group", "lang": "en"}], "type": "contact data set", "refObjectId": "ab62e83b-7504-48ae-abdc-def53c14790d", "uri": "../contacts/ab62e83b-7504-48ae-abdc-def53c14790d.xml"}, "copyright": true, "licenseType": "Free of charge for all users and uses", "accessRestrictions": [{"value": "None", "lang": "en"}], "other": {"anies": [{"name": "referenceToPublisher", "value": {"shortDescription": [{"value": "Institut Bauen und Umwelt e. V.", "lang": "en"}], "type": "contact data set", "refObjectId": "d111dbec-b024-4be5-86c5-752d6eb2cf95", "uri": "../contacts/d111dbec-b024-4be5-86c5-752d6eb2cf95.xml"}}]}}}, "exchanges": {"exchange": [{"dataSetInternalID": 0, "referenceToFlowDataSet": {"shortDescription": [{"value": "Window operator for VELUX GGL/GGU (KMG 100K) and control system (KUX 110), mains connected (Fensterantrieb für VELUX GGL/GGU (KMG 100K) und kontrollsystem (KUX 110), grid)", "lang": "en"}], "type": "flow data set", "refObjectId": "8e0499bf-21e4-bcdf-99d4-18dcde9bdf48", "uri": "../flows/8e0499bf-21e4-bcdf-99d4-18dcde9bdf48.xml"}, "meanAmount": 1.0, "referencesToDataSource": {}, "referenceFlow": true, "resolvedFlowVersion": "00.03.000", "resultingflowAmount": 1.0, "flowProperties": [{"name": [{"lang": "en", "value": "Number of pieces"}, {"lang": "de", "value": "Anzahl"}], "uuid": "01846770-4cfe-4a25-8ad9-919d8d378345", "referenceFlowProperty": true, "meanValue": 1.0, "referenceUnit": "pcs.", "unitGroupUUID": "934110e3-baf4-49e9-992c-3d8109a6aafb"}], "materialProperties": [{"name": "mass reference", "value": "1.93", "unit": "kg/m^3", "unitDescription": "Kilogram per cubic meter "}], "typeOfFlow": "Product flow", "classification": {"classHierarchy": "Komponenten von Fenstern und Vorhangfassaden / Antriebssysteme / elektrisch", "name": "OEKOBAU.DAT"}}, {"dataSetInternalID": 1, "referenceToFlowDataSet": {"shortDescription": [{"value": "Renewable primary energy as energy carrier (PERE)", "lang": "en"}, {"value": "Erneuerbare Primärenergie als Energieträger (PERE)", "lang": "de"}], "type": "flow data set", "refObjectId": "20f32be5-0398-4288-9b6d-accddd195317", "uri": "../flows/20f32be5-0398-4288-9b6d-accddd195317.xml"}, "exchange direction": "INPUT", "other": {"anies": [{"name": "referenceToUnitGroupDataSet", "value": {"shortDescription": [{"value": "MJ", "lang": "en"}], "type": "unit group data set", "refObjectId": "93a60a57-a3c8-11da-a746-0800200c9a66", "uri": "../unitgroups/93a60a57-a3c8-11da-a746-0800200c9a66.xml"}}, {"value": "29.430457231997", "module": "A1"}, {"value": "0.124942111550557", "module": "A2"}, {"value": "17.25824953845", "module": "A3"}, {"value": "0", "module": "C1"}, {"value": "0.00652574933886473", "module": "C2"}, {"value": "0.776918337913675", "module": "C3"}, {"value": "2.70272588186204E-05", "module": "C4"}, {"value": "-4.05219354565851", "module": "D"}]}, "resolvedFlowVersion": "38.00.000", "flowProperties": [], "typeOfFlow": "Other flow", "classification": {"classHierarchy": "Quantities", "name": "GaBiCategories"}}, {"dataSetInternalID": 2, "referenceToFlowDataSet": {"shortDescription": [{"value": "Renewable primary energy resources as material utilization (PERM)", "lang": "en"}, {"value": "Erneuerbare Primärenergie zur stofflichen Nutzung (PERM)", "lang": "de"}], "type": "flow data set", "refObjectId": "fb3ec0de-548d-4508-aea5-00b73bf6f702", "uri": "../flows/fb3ec0de-548d-4508-aea5-00b73bf6f702.xml"}, "exchange direction": "INPUT", "other": {"anies": [{"name": "referenceToUnitGroupDataSet", "value": {"shortDescription": [{"value": "MJ", "lang": "en"}], "type": "unit group data set", "refObjectId": "93a60a57-a3c8-11da-a746-0800200c9a66", "uri": "../unitgroups/93a60a57-a3c8-11da-a746-0800200c9a66.xml"}}, {"value": "0", "module": "A1"}, {"value": "0", "module": "A2"}, {"value": "0", "module": "A3"}, {"value": "0", "module": "C1"}, {"value": "0", "module": "C2"}, {"value": "0", "module": "C3"}, {"value": "0", "module": "C4"}, {"value": "0", "module": "D"}]}, "resolvedFlowVersion": "38.00.000", "flowProperties": [], "typeOfFlow": "Other flow", "classification": {"classHierarchy": "Quantities", "name": "GaBiCategories"}}, {"dataSetInternalID": 3, "referenceToFlowDataSet": {"shortDescription": [{"value": "Total use of renewable primary energy resources (PERT)", "lang": "en"}, {"value": "Total erneuerbare Primärenergie (PERT)", "lang": "de"}], "type": "flow data set", "refObjectId": "53f97275-fa8a-4cdd-9024-65936002acd0", "uri": "../flows/53f97275-fa8a-4cdd-9024-65936002acd0.xml"}, "exchange direction": "INPUT", "other": {"anies": [{"name": "referenceToUnitGroupDataSet", "value": {"shortDescription": [{"value": "MJ", "lang": "en"}], "type": "unit group data set", "refObjectId": "93a60a57-a3c8-11da-a746-0800200c9a66", "uri": "../unitgroups/93a60a57-a3c8-11da-a746-0800200c9a66.xml"}}, {"value": "29.430457231997", "module": "A1"}, {"value": "0.124942111550557", "module": "A2"}, {"value": "17.25824953845", "module": "A3"}, {"value": "0", "module": "C1"}, {"value": "0.00652574933886473", "module": "C2"}, {"value": "0.776918337913675", "module": "C3"}, {"value": "2.70272588186204E-05", "module": "C4"}, {"value": "-4.05219354565851", "module": "D"}]}, "resolvedFlowVersion": "38.00.000", "flowProperties": [], "typeOfFlow": "Other flow", "classification": {"classHierarchy": "Quantities / Environmental quantities / EPD EN 15804 / LCI indicators", "name": "GaBiCategories"}}, {"dataSetInternalID": 4, "referenceToFlowDataSet": {"shortDescription": [{"value": "Non renewable primary energy as energy carrier (PENRE)", "lang": "en"}, {"value": "Nicht-erneuerbare Primärenergie als Energieträger (PENRE)", "lang": "de"}], "type": "flow data set", "refObjectId": "ac857178-2b45-46ec-892a-a9a4332f0372", "uri": "../flows/ac857178-2b45-46ec-892a-a9a4332f0372.xml"}, "exchange direction": "INPUT", "other": {"anies": [{"name": "referenceToUnitGroupDataSet", "value": {"shortDescription": [{"value": "MJ", "lang": "en"}], "type": "unit group data set", "refObjectId": "93a60a57-a3c8-11da-a746-0800200c9a66", "uri": "../unitgroups/93a60a57-a3c8-11da-a746-0800200c9a66.xml"}}, {"value": "153.278598272605", "module": "A1"}, {"value": "5.60714354430261", "module": "A2"}, {"value": "19.0981742291193", "module": "A3"}, {"value": "0", "module": "C1"}, {"value": "0.117089894246218", "module": "C2"}, {"value": "20.0756700427194", "module": "C3"}, {"value": "0.000200739248837281", "module": "C4"}, {"value": "-19.014825178646", "module": "D"}]}, "resolvedFlowVersion": "38.00.000", "flowProperties": [], "typeOfFlow": "Other flow", "classification": {"classHierarchy": "Quantities", "name": "GaBiCategories"}}, {"dataSetInternalID": 5, "referenceToFlowDataSet": {"shortDescription": [{"value": "Non renewable primary energy as material utilization (PENRM)", "lang": "en"}, {"value": "Nicht-erneuerbare Primärenergie zur stofflichen Nutzung (PENRM)", "lang": "de"}], "type": "flow data set", "refObjectId": "1421caa0-679d-4bf4-b282-0eb850ccae27", "uri": "../flows/1421caa0-679d-4bf4-b282-0eb850ccae27.xml"}, "exchange direction": "INPUT", "other": {"anies": [{"name": "referenceToUnitGroupDataSet", "value": {"shortDescription": [{"value": "MJ", "lang": "en"}], "type": "unit group data set", "refObjectId": "93a60a57-a3c8-11da-a746-0800200c9a66", "uri": "../unitgroups/93a60a57-a3c8-11da-a746-0800200c9a66.xml"}}, {"value": "23.2926689127196", "module": "A1"}, {"value": "0", "module": "A2"}, {"value": "8.236", "module": "A3"}, {"value": "0", "module": "C1"}, {"value": "0", "module": "C2"}, {"value": "-17.5973", "module": "C3"}, {"value": "0", "module": "C4"}, {"value": "0", "module": "D"}]}, "resolvedFlowVersion": "38.00.000", "flowProperties": [], "typeOfFlow": "Other flow", "classification": {"classHierarchy": "Quantities", "name": "GaBiCategories"}}, {"dataSetInternalID": 6, "referenceToFlowDataSet": {"shortDescription": [{"value": "Total use of non renewable primary energy resources (PENRT)", "lang": "en"}, {"value": "Total nicht erneuerbare Primärenergie (PENRT)", "lang": "de"}], "type": "flow data set", "refObjectId": "06159210-646b-4c8d-8583-da9b3b95a6c1", "uri": "../flows/06159210-646b-4c8d-8583-da9b3b95a6c1.xml"}, "exchange direction": "INPUT", "other": {"anies": [{"name": "referenceToUnitGroupDataSet", "value": {"shortDescription": [{"value": "MJ", "lang": "en"}], "type": "unit group data set", "refObjectId": "93a60a57-a3c8-11da-a746-0800200c9a66", "uri": "../unitgroups/93a60a57-a3c8-11da-a746-0800200c9a66.xml"}}, {"value": "176.571272068228", "module": "A1"}, {"value": "5.60714354430263", "module": "A2"}, {"value": "27.3341742291197", "module": "A3"}, {"value": "0", "module": "C1"}, {"value": "0.117089894246218", "module": "C2"}, {"value": "2.47837635783299", "module": "C3"}, {"value": "0.000200739248837285", "module": "C4"}, {"value": "-19.0148251786464", "module": "D"}]}, "resolvedFlowVersion": "38.00.000", "flowProperties": [], "typeOfFlow": "Other flow", "classification": {"classHierarchy": "Quantities / Environmental quantities / EPD EN 15804 / LCI indicators", "name": "GaBiCategories"}}, {"dataSetInternalID": 7, "referenceToFlowDataSet": {"shortDescription": [{"value": "Use of secondary material (SM)", "lang": "en"}, {"value": "Einsatz von Sekundärstoffen (SM)", "lang": "de"}], "type": "flow data set", "refObjectId": "c6a1f35f-2d09-4f54-8dfb-97e502e1ce92", "uri": "../flows/c6a1f35f-2d09-4f54-8dfb-97e502e1ce92.xml"}, "exchange direction": "INPUT", "other": {"anies": [{"name": "referenceToUnitGroupDataSet", "value": {"shortDescription": [{"value": "kg", "lang": "en"}], "type": "unit group data set", "refObjectId": "ad38d542-3fe9-439d-9b95-2f5f7752acaf", "uri": "../unitgroups/ad38d542-3fe9-439d-9b95-2f5f7752acaf.xml"}}, {"value": "0.1785828", "module": "A1"}, {"value": "0", "module": "A2"}, {"value": "0", "module": "A3"}, {"value": "0", "module": "C1"}, {"value": "0", "module": "C2"}, {"value": "0", "module": "C3"}, {"value": "0", "module": "C4"}, {"value": "0", "module": "D"}]}, "resolvedFlowVersion": "38.00.000", "flowProperties": [], "typeOfFlow": "Other flow", "classification": {"classHierarchy": "Quantities / Environmental quantities / EPD EN 15804 / LCI indicators", "name": "GaBiCategories"}}, {"dataSetInternalID": 8, "referenceToFlowDataSet": {"shortDescription": [{"value": "Use of renewable secondary fuels (RSF)", "lang": "en"}, {"value": "Erneuerbare Sekundärbrennstoffe (RSF)", "lang": "de"}], "type": "flow data set", "refObjectId": "64333088-a55f-4aa2-9a31-c10b07816787", "uri": "../flows/64333088-a55f-4aa2-9a31-c10b07816787.xml"}, "exchange direction": "INPUT", "other": {"anies": [{"name": "referenceToUnitGroupDataSet", "value": {"shortDescription": [{"value": "MJ", "lang": "en"}], "type": "unit group data set", "refObjectId": "93a60a57-a3c8-11da-a746-0800200c9a66", "uri": "../unitgroups/93a60a57-a3c8-11da-a746-0800200c9a66.xml"}}, {"value": "0", "module": "A1"}, {"value": "0", "module": "A2"}, {"value": "0", "module": "A3"}, {"value": "0", "module": "C1"}, {"value": "0", "module": "C2"}, {"value": "0", "module": "C3"}, {"value": "0", "module": "C4"}, {"value": "0", "module": "D"}]}, "resolvedFlowVersion": "38.00.000", "flowProperties": [], "typeOfFlow": "Other flow", "classification": {"classHierarchy": "Quantities / Environmental quantities / EPD EN 15804 / LCI indicators", "name": "GaBiCategories"}}, {"dataSetInternalID": 9, "referenceToFlowDataSet": {"shortDescription": [{"value": "Use of non renewable secondary fuels (NRSF)", "lang": "en"}, {"value": "Nicht erneuerbare Sekundärbrennstoffe (NRSF)", "lang": "de"}], "type": "flow data set", "refObjectId": "89def144-d39a-4287-b86f-efde453ddcb2", "uri": "../flows/89def144-d39a-4287-b86f-efde453ddcb2.xml"}, "exchange direction": "INPUT", "other": {"anies": [{"name": "referenceToUnitGroupDataSet", "value": {"shortDescription": [{"value": "MJ", "lang": "en"}], "type": "unit group data set", "refObjectId": "93a60a57-a3c8-11da-a746-0800200c9a66", "uri": "../unitgroups/93a60a57-a3c8-11da-a746-0800200c9a66.xml"}}, {"value": "0", "module": "A1"}, {"value": "0", "module": "A2"}, {"value": "0", "module": "A3"}, {"value": "0", "module": "C1"}, {"value": "0", "module": "C2"}, {"value": "0", "module": "C3"}, {"value": "0", "module": "C4"}, {"value": "0", "module": "D"}]}, "resolvedFlowVersion": "38.00.000", "flowProperties": [], "typeOfFlow": "Other flow", "classification": {"classHierarchy": "Quantities / Environmental quantities / EPD EN 15804 / LCI indicators", "name": "GaBiCategories"}}, {"dataSetInternalID": 10, "referenceToFlowDataSet": {"shortDescription": [{"value": "Use of net fresh water (FW)", "lang": "en"}, {"value": "Einsatz von Süßwasserressourcen (FW)", "lang": "de"}], "type": "flow data set", "refObjectId": "3cf952c8-f3a4-461d-8c96-96456ca62246", "uri": "../flows/3cf952c8-f3a4-461d-8c96-96456ca62246.xml"}, "exchange direction": "INPUT", "other": {"anies": [{"name": "referenceToUnitGroupDataSet", "value": {"shortDescription": [{"value": "m^3", "lang": "en"}], "type": "unit group data set", "refObjectId": "cd950537-0a98-4044-9ba7-9f9a68d0a504", "uri": "../unitgroups/cd950537-0a98-4044-9ba7-9f9a68d0a504.xml"}}, {"value": "0.128732151373393", "module": "A1"}, {"value": "0.000148964249570617", "module": "A2"}, {"value": "0.00785384009858048", "module": "A3"}, {"value": "0", "module": "C1"}, {"value": "7.46974582288681E-06", "module": "C2"}, {"value": "0.0120952543379517", "module": "C3"}, {"value": "4.95169370233256E-08", "module": "C4"}, {"value": "-0.0112745897817188", "module": "D"}]}, "resolvedFlowVersion": "38.00.000", "flowProperties": [], "typeOfFlow": "Other flow", "classification": {"classHierarchy": "Quantities / Environmental quantities / EPD EN 15804 / LCI indicators", "name": "GaBiCategories"}}, {"dataSetInternalID": 11, "referenceToFlowDataSet": {"shortDescription": [{"value": "Hazardous waste disposed (HWD)", "lang": "en"}, {"value": "Gefährlicher Abfall zur Deponie (HWD)", "lang": "de"}], "type": "flow data set", "refObjectId": "430f9e0f-59b2-46a0-8e0d-55e0e84948fc", "uri": "../flows/430f9e0f-59b2-46a0-8e0d-55e0e84948fc.xml"}, "exchange direction": "OUTPUT", "other": {"anies": [{"name": "referenceToUnitGroupDataSet", "value": {"shortDescription": [{"value": "kg", "lang": "en"}], "type": "unit group data set", "refObjectId": "ad38d542-3fe9-439d-9b95-2f5f7752acaf", "uri": "../unitgroups/ad38d542-3fe9-439d-9b95-2f5f7752acaf.xml"}}, {"value": "0.000258263655661161", "module": "A1"}, {"value": "1.29646430241887E-10", "module": "A2"}, {"value": "0.000134556685981633", "module": "A3"}, {"value": "0", "module": "C1"}, {"value": "5.90008566923441E-12", "module": "C2"}, {"value": "5.49881425066653E-10", "module": "C3"}, {"value": "2.13133544122176E-14", "module": "C4"}, {"value": "-2.97151254938661E-09", "module": "D"}]}, "resolvedFlowVersion": "38.00.000", "flowProperties": [], "typeOfFlow": "Other flow", "classification": {"classHierarchy": "Quantities / Environmental quantities / EPD EN 15804 / LCI indicators", "name": "GaBiCategories"}}, {"dataSetInternalID": 12, "referenceToFlowDataSet": {"shortDescription": [{"value": "Non hazardous waste disposed (NHWD)", "lang": "en"}, {"value": "Entsorgter nicht gefährlicher Abfall (NHWD)", "lang": "de"}], "type": "flow data set", "refObjectId": "b29ef66b-e286-4afa-949f-62f1a7b4d7fa", "uri": "../flows/b29ef66b-e286-4afa-949f-62f1a7b4d7fa.xml"}, "exchange direction": "OUTPUT", "other": {"anies": [{"name": "referenceToUnitGroupDataSet", "value": {"shortDescription": [{"value": "kg", "lang": "en"}], "type": "unit group data set", "refObjectId": "ad38d542-3fe9-439d-9b95-2f5f7752acaf", "uri": "../unitgroups/ad38d542-3fe9-439d-9b95-2f5f7752acaf.xml"}}, {"value": "0.617378425534397", "module": "A1"}, {"value": "0.000660037439338458", "module": "A2"}, {"value": "0.0361195575360383", "module": "A3"}, {"value": "0", "module": "C1"}, {"value": "1.73939029546622E-05", "module": "C2"}, {"value": "0.122936442488623", "module": "C3"}, {"value": "0.00100098330108138", "module": "C4"}, {"value": "-0.0513035005057987", "module": "D"}]}, "resolvedFlowVersion": "38.00.000", "flowProperties": [], "typeOfFlow": "Other flow", "classification": {"classHierarchy": "Quantities / Environmental quantities / EPD EN 15804 / LCI indicators", "name": "GaBiCategories"}}, {"dataSetInternalID": 13, "referenceToFlowDataSet": {"shortDescription": [{"value": "Radioactive waste disposed (RWD)", "lang": "en"}, {"value": "Entsorgter radioaktiver Abfall (RWD)", "lang": "de"}], "type": "flow data set", "refObjectId": "3449546e-52ad-4b39-b809-9fb77cea8ff6", "uri": "../flows/3449546e-52ad-4b39-b809-9fb77cea8ff6.xml"}, "exchange direction": "OUTPUT", "other": {"anies": [{"name": "referenceToUnitGroupDataSet", "value": {"shortDescription": [{"value": "kg", "lang": "en"}], "type": "unit group data set", "refObjectId": "ad38d542-3fe9-439d-9b95-2f5f7752acaf", "uri": "../unitgroups/ad38d542-3fe9-439d-9b95-2f5f7752acaf.xml"}}, {"value": "0.00317173634747159", "module": "A1"}, {"value": "6.43181810523711E-06", "module": "A2"}, {"value": "0.00132594148244663", "module": "A3"}, {"value": "0", "module": "C1"}, {"value": "1.41634962679595E-07", "module": "C2"}, {"value": "0.000228611962653546", "module": "C3"}, {"value": "2.10733007556803E-09", "module": "C4"}, {"value": "-0.000903388994891286", "module": "D"}]}, "resolvedFlowVersion": "38.00.000", "flowProperties": [], "typeOfFlow": "Other flow", "classification": {"classHierarchy": "Quantities / Environmental quantities / EPD EN 15804 / LCI indicators", "name": "GaBiCategories"}}, {"dataSetInternalID": 14, "referenceToFlowDataSet": {"shortDescription": [{"value": "Components for re-use (CRU)", "lang": "en"}, {"value": "Komponenten für die Wiederverwendung (CRU)", "lang": "de"}], "type": "flow data set", "refObjectId": "a2b32f97-3fc7-4af2-b209-525bc6426f33", "uri": "../flows/a2b32f97-3fc7-4af2-b209-525bc6426f33.xml"}, "exchange direction": "OUTPUT", "other": {"anies": [{"name": "referenceToUnitGroupDataSet", "value": {"shortDescription": [{"value": "kg", "lang": "en"}], "type": "unit group data set", "refObjectId": "ad38d542-3fe9-439d-9b95-2f5f7752acaf", "uri": "../unitgroups/ad38d542-3fe9-439d-9b95-2f5f7752acaf.xml"}}, {"value": "0", "module": "A1"}, {"value": "0", "module": "A2"}, {"value": "0", "module": "A3"}, {"value": "0", "module": "C1"}, {"value": "0", "module": "C2"}, {"value": "0", "module": "C3"}, {"value": "0", "module": "C4"}, {"value": "0", "module": "D"}]}, "resolvedFlowVersion": "38.00.000", "flowProperties": [], "typeOfFlow": "Other flow", "classification": {"classHierarchy": "Quantities / Environmental quantities / EPD EN 15804 / LCI indicators", "name": "GaBiCategories"}}, {"dataSetInternalID": 15, "referenceToFlowDataSet": {"shortDescription": [{"value": "Materials for recycling (MFR)", "lang": "en"}, {"value": "Stoffe zum Recycling (MFR)", "lang": "de"}], "type": "flow data set", "refObjectId": "d7fe48a5-4103-49c8-9aae-b0b5dfdbd6ae", "uri": "../flows/d7fe48a5-4103-49c8-9aae-b0b5dfdbd6ae.xml"}, "exchange direction": "OUTPUT", "other": {"anies": [{"name": "referenceToUnitGroupDataSet", "value": {"shortDescription": [{"value": "kg", "lang": "en"}], "type": "unit group data set", "refObjectId": "ad38d542-3fe9-439d-9b95-2f5f7752acaf", "uri": "../unitgroups/ad38d542-3fe9-439d-9b95-2f5f7752acaf.xml"}}, {"value": "0", "module": "A1"}, {"value": "0", "module": "A2"}, {"value": "0", "module": "A3"}, {"value": "0", "module": "C1"}, {"value": "0", "module": "C2"}, {"value": "0.69624", "module": "C3"}, {"value": "0", "module": "C4"}, {"value": "0", "module": "D"}]}, "resolvedFlowVersion": "38.00.000", "flowProperties": [], "typeOfFlow": "Other flow", "classification": {"classHierarchy": "Quantities / Environmental quantities / EPD EN 15804 / LCI indicators", "name": "GaBiCategories"}}, {"dataSetInternalID": 16, "referenceToFlowDataSet": {"shortDescription": [{"value": "Materials for energy recovery (MER)", "lang": "en"}, {"value": "Stoffe für die Energierückgewinnung (MER)", "lang": "de"}], "type": "flow data set", "refObjectId": "59a9181c-3aaf-46ee-8b13-2b3723b6e447", "uri": "../flows/59a9181c-3aaf-46ee-8b13-2b3723b6e447.xml"}, "exchange direction": "OUTPUT", "other": {"anies": [{"name": "referenceToUnitGroupDataSet", "value": {"shortDescription": [{"value": "kg", "lang": "en"}], "type": "unit group data set", "refObjectId": "ad38d542-3fe9-439d-9b95-2f5f7752acaf", "uri": "../unitgroups/ad38d542-3fe9-439d-9b95-2f5f7752acaf.xml"}}, {"value": "0", "module": "A1"}, {"value": "0", "module": "A2"}, {"value": "0", "module": "A3"}, {"value": "0", "module": "C1"}, {"value": "0", "module": "C2"}, {"value": "0.6708", "module": "C3"}, {"value": "0", "module": "C4"}, {"value": "0", "module": "D"}]}, "resolvedFlowVersion": "38.00.000", "flowProperties": [], "typeOfFlow": "Other flow", "classification": {"classHierarchy": "Quantities / Environmental quantities / EPD EN 15804 / LCI indicators", "name": "GaBiCategories"}}, {"dataSetInternalID": 17, "referenceToFlowDataSet": {"shortDescription": [{"value": "Exported electrical energy (EEE)", "lang": "en"}, {"value": "Exportierte elektrische Energie (EEE)", "lang": "de"}], "type": "flow data set", "refObjectId": "4da0c987-2b76-40d6-9e9e-82a017aaaf29", "uri": "../flows/4da0c987-2b76-40d6-9e9e-82a017aaaf29.xml"}, "exchange direction": "OUTPUT", "other": {"anies": [{"name": "referenceToUnitGroupDataSet", "value": {"shortDescription": [{"value": "MJ", "lang": "en"}], "type": "unit group data set", "refObjectId": "93a60a57-a3c8-11da-a746-0800200c9a66", "uri": "../unitgroups/93a60a57-a3c8-11da-a746-0800200c9a66.xml"}}, {"value": "0", "module": "A1"}, {"value": "0", "module": "A2"}, {"value": "0", "module": "A3"}, {"value": "0", "module": "C1"}, {"value": "0", "module": "C2"}, {"value": "0", "module": "C3"}, {"value": "0", "module": "C4"}, {"value": "2.62633548812355", "module": "D"}]}, "resolvedFlowVersion": "38.00.000", "flowProperties": [], "typeOfFlow": "Other flow", "classification": {"classHierarchy": "Quantities / Environmental quantities / EPD EN 15804 / LCI indicators", "name": "GaBiCategories"}}, {"dataSetInternalID": 18, "referenceToFlowDataSet": {"shortDescription": [{"value": "Exported thermal energy (EET)", "lang": "en"}, {"value": "Exportierte thermische Energie (EET)", "lang": "de"}], "type": "flow data set", "refObjectId": "98daf38a-7a79-46d3-9a37-2b7bd0955810", "uri": "../flows/98daf38a-7a79-46d3-9a37-2b7bd0955810.xml"}, "exchange direction": "OUTPUT", "other": {"anies": [{"name": "referenceToUnitGroupDataSet", "value": {"shortDescription": [{"value": "MJ", "lang": "en"}], "type": "unit group data set", "refObjectId": "93a60a57-a3c8-11da-a746-0800200c9a66", "uri": "../unitgroups/93a60a57-a3c8-11da-a746-0800200c9a66.xml"}}, {"value": "0", "module": "A1"}, {"value": "0", "module": "A2"}, {"value": "0", "module": "A3"}, {"value": "0", "module": "C1"}, {"value": "0", "module": "C2"}, {"value": "0", "module": "C3"}, {"value": "0", "module": "C4"}, {"value": "4.74996528508744", "module": "D"}]}, "resolvedFlowVersion": "38.00.000", "flowProperties": [], "typeOfFlow": "Other flow", "classification": {"classHierarchy": "Quantities / Environmental quantities / EPD EN 15804 / LCI indicators", "name": "GaBiCategories"}}]}, "LCIAResults": {"LCIAResult": [{"referenceToLCIAMethodDataSet": {"shortDescription": [{"value": "Global Warming Potential total (GWP-total)", "lang": "en"}, {"value": "Globales Erwärmungspotenzial total (GWP-total)", "lang": "de"}], "type": "LCIA method data set", "refObjectId": "6a37f984-a4b3-458a-a20a-64418c145fa2", "uri": "../lciamethods/6a37f984-a4b3-458a-a20a-64418c145fa2.xml"}, "other": {"anies": [{"name": "referenceToUnitGroupDataSet", "value": {"shortDescription": [{"value": "kg CO_(2) eq", "lang": "en"}], "type": "unit group data set", "refObjectId": "1ebf3012-d0db-4de2-aefd-ef30cedb0be1", "uri": "../unitgroups/1ebf3012-d0db-4de2-aefd-ef30cedb0be1.xml"}}, {"value": "11.4522388967991", "module": "A1"}, {"value": "0.448944992525014", "module": "A2"}, {"value": "0.733178405587394", "module": "A3"}, {"value": "0", "module": "C1"}, {"value": "0.00884718826363946", "module": "C2"}, {"value": "1.6686947400564", "module": "C3"}, {"value": "1.47277312572022E-05", "module": "C4"}, {"value": "-1.36020548697556", "module": "D"}]}}, {"referenceToLCIAMethodDataSet": {"shortDescription": [{"value": "Global Warming Potential fossil fuels (GWP-fossil)", "lang": "en"}, {"value": "Globales Erwärmungspotenzial fossil (GWP-fossil)", "lang": "de"}], "type": "LCIA method data set", "refObjectId": "5f635281-343e-44fb-83df-1971b155e6b6", "uri": "../lciamethods/5f635281-343e-44fb-83df-1971b155e6b6.xml"}, "other": {"anies": [{"name": "referenceToUnitGroupDataSet", "value": {"shortDescription": [{"value": "kg CO_(2) eq", "lang": "en"}], "type": "unit group data set", "refObjectId": "1ebf3012-d0db-4de2-aefd-ef30cedb0be1", "uri": "../unitgroups/1ebf3012-d0db-4de2-aefd-ef30cedb0be1.xml"}}, {"value": "11.5681173152594", "module": "A1"}, {"value": "0.447508588092537", "module": "A2"}, {"value": "1.35977181087792", "module": "A3"}, {"value": "0", "module": "C1"}, {"value": "0.00878645889734394", "module": "C2"}, {"value": "1.66723266583735", "module": "C3"}, {"value": "1.51226960448363E-05", "module": "C4"}, {"value": "-1.35812017383514", "module": "D"}]}}, {"referenceToLCIAMethodDataSet": {"shortDescription": [{"value": "Global Warming Potential biogenic (GWP-biogenic)", "lang": "en"}, {"value": "Globales Erwärmungspotenzial biogen (GWP-biogenic)", "lang": "de"}], "type": "LCIA method data set", "refObjectId": "2356e1ab-0185-4db5-86e5-16de51c7485c", "uri": "../lciamethods/2356e1ab-0185-4db5-86e5-16de51c7485c.xml"}, "other": {"anies": [{"name": "referenceToUnitGroupDataSet", "value": {"shortDescription": [{"value": "kg CO_(2) eq", "lang": "en"}], "type": "unit group data set", "refObjectId": "1ebf3012-d0db-4de2-aefd-ef30cedb0be1", "uri": "../unitgroups/1ebf3012-d0db-4de2-aefd-ef30cedb0be1.xml"}}, {"value": "-0.132034611152866", "module": "A1"}, {"value": "0.000188649579278884", "module": "A2"}, {"value": "-0.627787099578181", "module": "A3"}, {"value": "0", "module": "C1"}, {"value": "-1.12044494877962E-05", "module": "C2"}, {"value": "0.00128345299244659", "module": "C3"}, {"value": "-4.39399250511205E-07", "module": "C4"}, {"value": "-0.000540580274231303", "module": "D"}]}}, {"referenceToLCIAMethodDataSet": {"shortDescription": [{"value": "Global Warming Potential luluc (GWP-luluc)", "lang": "en"}, {"value": "Globales Erwärmungspotenzial luluc (GWP-luluc)", "lang": "de"}], "type": "LCIA method data set", "refObjectId": "4331bbdb-978a-490d-8707-eeb047f01a55", "uri": "../lciamethods/4331bbdb-978a-490d-8707-eeb047f01a55.xml"}, "other": {"anies": [{"name": "referenceToUnitGroupDataSet", "value": {"shortDescription": [{"value": "kg CO_(2) eq", "lang": "en"}], "type": "unit group data set", "refObjectId": "1ebf3012-d0db-4de2-aefd-ef30cedb0be1", "uri": "../unitgroups/1ebf3012-d0db-4de2-aefd-ef30cedb0be1.xml"}}, {"value": "0.0161561926925837", "module": "A1"}, {"value": "0.00124775485319847", "module": "A2"}, {"value": "0.0011936942876542", "module": "A3"}, {"value": "0", "module": "C1"}, {"value": "7.19338157833183E-05", "module": "C2"}, {"value": "0.000178621226601911", "module": "C3"}, {"value": "4.44344628770165E-08", "module": "C4"}, {"value": "-0.00154473286618214", "module": "D"}]}}, {"referenceToLCIAMethodDataSet": {"shortDescription": [{"value": "Depletion potential of the stratospheric ozone layer (ODP)", "lang": "en"}, {"value": "Abbau Potential der stratosphärischen Ozonschicht (ODP)", "lang": "de"}], "type": "LCIA method data set", "refObjectId": "b5c629d6-def3-11e6-bf01-fe55135034f3", "uri": "../lciamethods/b5c629d6-def3-11e6-bf01-fe55135034f3.xml"}, "other": {"anies": [{"name": "referenceToUnitGroupDataSet", "value": {"shortDescription": [{"value": "kg CFC11 eq", "lang": "en"}], "type": "unit group data set", "refObjectId": "d9e957c9-7309-4474-bf3a-7777df6c4e5b", "uri": "../unitgroups/d9e957c9-7309-4474-bf3a-7777df6c4e5b.xml"}}, {"value": "1.37294322055507E-09", "module": "A1"}, {"value": "4.97743950593712E-17", "module": "A2"}, {"value": "1.94879340590823E-11", "module": "A3"}, {"value": "0", "module": "C1"}, {"value": "1.12230329175202E-18", "module": "C2"}, {"value": "6.17263248723611E-09", "module": "C3"}, {"value": "5.87705361389726E-20", "module": "C4"}, {"value": "-8.12575997402492E-15", "module": "D"}]}}, {"referenceToLCIAMethodDataSet": {"shortDescription": [{"value": "Acidification potential of land and water (AP)", "lang": "en"}, {"value": "Versauerungspotenzial von Boden und Wasser (AP)", "lang": "de"}], "type": "LCIA method data set", "refObjectId": "b5c611c6-def3-11e6-bf01-fe55135034f3", "uri": "../lciamethods/b5c611c6-def3-11e6-bf01-fe55135034f3.xml"}, "other": {"anies": [{"name": "referenceToUnitGroupDataSet", "value": {"shortDescription": [{"value": "mol H^(+) eq", "lang": "en"}], "type": "unit group data set", "refObjectId": "42e089ac-92bf-4bf2-8ca1-5fc40d18f2ed", "uri": "../unitgroups/42e089ac-92bf-4bf2-8ca1-5fc40d18f2ed.xml"}}, {"value": "0.0512717466577109", "module": "A1"}, {"value": "0.0113419361224135", "module": "A2"}, {"value": "0.00407384330234916", "module": "A3"}, {"value": "0", "module": "C1"}, {"value": "2.74640120670846E-05", "module": "C2"}, {"value": "0.00190333449746383", "module": "C3"}, {"value": "1.07716154589491E-07", "module": "C4"}, {"value": "-0.00420528796860076", "module": "D"}]}}, {"referenceToLCIAMethodDataSet": {"shortDescription": [{"value": "Eutrophication potential aquatic freshwater (EP-freshwater)", "lang": "en"}, {"value": "Eutrophierungspotenzial Süßwasser (EP-freshwater)", "lang": "de"}], "type": "LCIA method data set", "refObjectId": "b53ec18f-7377-4ad3-86eb-cc3f4f276b2b", "uri": "../lciamethods/b53ec18f-7377-4ad3-86eb-cc3f4f276b2b.xml"}, "other": {"anies": [{"name": "referenceToUnitGroupDataSet", "value": {"shortDescription": [{"value": "kg P eq", "lang": "en"}], "type": "unit group data set", "refObjectId": "0429039d-a61d-4590-ba67-aa4a20a810a1", "uri": "../unitgroups/0429039d-a61d-4590-ba67-aa4a20a810a1.xml"}}, {"value": "0.000159182133030732", "module": "A1"}, {"value": "5.16474813143236E-07", "module": "A2"}, {"value": "1.56343977901255E-05", "module": "A3"}, {"value": "0", "module": "C1"}, {"value": "2.60766172149279E-08", "module": "C2"}, {"value": "1.03369004724513E-05", "module": "C3"}, {"value": "2.53876691215396E-11", "module": "C4"}, {"value": "-1.35565073665037E-06", "module": "D"}]}}, {"referenceToLCIAMethodDataSet": {"shortDescription": [{"value": "Eutrophication potential aquatic marine (EP-marine)", "lang": "en"}, {"value": "Eutrophierungspotenzial Salzwasser (EP-marine)", "lang": "de"}], "type": "LCIA method data set", "refObjectId": "b5c619fa-def3-11e6-bf01-fe55135034f3", "uri": "../lciamethods/b5c619fa-def3-11e6-bf01-fe55135034f3.xml"}, "other": {"anies": [{"name": "referenceToUnitGroupDataSet", "value": {"shortDescription": [{"value": "kg N eq", "lang": "en"}], "type": "unit group data set", "refObjectId": "d05bb823-ecdf-4686-8c40-bf1d9257859f", "uri": "../unitgroups/d05bb823-ecdf-4686-8c40-bf1d9257859f.xml"}}, {"value": "0.00878089199690223", "module": "A1"}, {"value": "0.0030913125012211", "module": "A2"}, {"value": "0.00128534079562654", "module": "A3"}, {"value": "0", "module": "C1"}, {"value": "1.26260531182291E-05", "module": "C2"}, {"value": "0.000878915626589028", "module": "C3"}, {"value": "2.79593696984463E-08", "module": "C4"}, {"value": "-0.000714835468396519", "module": "D"}]}}, {"referenceToLCIAMethodDataSet": {"shortDescription": [{"value": "Eutrophication potential terrestrial (EP-terrestrial)", "lang": "en"}, {"value": "Eutrophierungspotenzial Land (EP-terrestrial)", "lang": "de"}], "type": "LCIA method data set", "refObjectId": "b5c614d2-def3-11e6-bf01-fe55135034f3", "uri": "../lciamethods/b5c614d2-def3-11e6-bf01-fe55135034f3.xml"}, "other": {"anies": [{"name": "referenceToUnitGroupDataSet", "value": {"shortDescription": [{"value": "mol N eq", "lang": "en"}], "type": "unit group data set", "refObjectId": "71b4d617-0ec9-4d3f-b65e-e438940c2401", "uri": "../unitgroups/71b4d617-0ec9-4d3f-b65e-e438940c2401.xml"}}, {"value": "0.0926635276270142", "module": "A1"}, {"value": "0.0339038303457573", "module": "A2"}, {"value": "0.0130526977357528", "module": "A3"}, {"value": "0", "module": "C1"}, {"value": "0.000141096042860177", "module": "C2"}, {"value": "0.00969308260778104", "module": "C3"}, {"value": "3.07183748616142E-07", "module": "C4"}, {"value": "-0.00770479331708566", "module": "D"}]}}, {"referenceToLCIAMethodDataSet": {"shortDescription": [{"value": "Formation potential of tropospheric ozone photochemical oxidants (POCP)", "lang": "en"}, {"value": "Bildungspotential für troposphärisches Ozon (POCP)", "lang": "de"}], "type": "LCIA method data set", "refObjectId": "b5c610fe-def3-11e6-bf01-fe55135034f3", "uri": "../lciamethods/b5c610fe-def3-11e6-bf01-fe55135034f3.xml"}, "other": {"anies": [{"name": "referenceToUnitGroupDataSet", "value": {"shortDescription": [{"value": "kg NMVOC eq", "lang": "en"}], "type": "unit group data set", "refObjectId": "d27c25f8-fbc1-44c6-b47b-4adbae4199c6", "uri": "../unitgroups/d27c25f8-fbc1-44c6-b47b-4adbae4199c6.xml"}}, {"value": "0.0277101622012216", "module": "A1"}, {"value": "0.00845848067966748", "module": "A2"}, {"value": "0.00378429391767015", "module": "A3"}, {"value": "0", "module": "C1"}, {"value": "2.47227382497972E-05", "module": "C2"}, {"value": "0.00225403054243565", "module": "C3"}, {"value": "8.4724483659545E-08", "module": "C4"}, {"value": "-0.00213401039156704", "module": "D"}]}}, {"referenceToLCIAMethodDataSet": {"shortDescription": [{"value": "Abiotic depletion potential for non fossil resources (ADPE)", "lang": "en"}, {"value": "Potenzial für den abiotischen Abbau nicht fossiler Ressourcen (ADPE)", "lang": "de"}], "type": "LCIA method data set", "refObjectId": "b2ad6494-c78d-11e6-9d9d-cec0c932ce01", "uri": "../lciamethods/b2ad6494-c78d-11e6-9d9d-cec0c932ce01.xml"}, "other": {"anies": [{"name": "referenceToUnitGroupDataSet", "value": {"shortDescription": [{"value": "kg Sb eq", "lang": "en"}], "type": "unit group data set", "refObjectId": "54ccd2d9-a32a-4fc2-923d-f2c8c93e89d4", "uri": "../unitgroups/54ccd2d9-a32a-4fc2-923d-f2c8c93e89d4.xml"}}, {"value": "0.000883566497983122", "module": "A1"}, {"value": "2.0405303132848E-08", "module": "A2"}, {"value": "2.01212599869587E-07", "module": "A3"}, {"value": "0", "module": "C1"}, {"value": "6.68756393926241E-10", "module": "C2"}, {"value": "2.0822199385351E-07", "module": "C3"}, {"value": "1.42725262330788E-12", "module": "C4"}, {"value": "-4.03430724970448E-05", "module": "D"}]}}, {"referenceToLCIAMethodDataSet": {"shortDescription": [{"value": "Abiotic depletion potential for fossil resources (ADPF)", "lang": "en"}, {"value": "Potenzial für den abiotischen Abbau fossiler Brennstoffe (ADPF)", "lang": "de"}], "type": "LCIA method data set", "refObjectId": "b2ad6110-c78d-11e6-9d9d-cec0c932ce01", "uri": "../lciamethods/b2ad6110-c78d-11e6-9d9d-cec0c932ce01.xml"}, "other": {"anies": [{"name": "referenceToUnitGroupDataSet", "value": {"shortDescription": [{"value": "MJ", "lang": "en"}], "type": "unit group data set", "refObjectId": "93a60a57-a3c8-11da-a746-0800200c9a66", "uri": "../unitgroups/93a60a57-a3c8-11da-a746-0800200c9a66.xml"}}, {"value": "176.52378265751", "module": "A1"}, {"value": "5.59979267404276", "module": "A2"}, {"value": "27.3275697402242", "module": "A3"}, {"value": "0", "module": "C1"}, {"value": "0.116933888061727", "module": "C2"}, {"value": "2.47775902456991", "module": "C3"}, {"value": "0.000200633380353006", "module": "C4"}, {"value": "-18.9957183169351", "module": "D"}]}}, {"referenceToLCIAMethodDataSet": {"shortDescription": [{"value": "Water use (WDP)", "lang": "en"}, {"value": "Wassernutzung (WDP)", "lang": "de"}], "type": "LCIA method data set", "refObjectId": "b2ad66ce-c78d-11e6-9d9d-cec0c932ce01", "uri": "../lciamethods/b2ad66ce-c78d-11e6-9d9d-cec0c932ce01.xml"}, "other": {"anies": [{"name": "referenceToUnitGroupDataSet", "value": {"shortDescription": [{"value": "m^(3) world eq deprived", "lang": "en"}], "type": "unit group data set", "refObjectId": "6ae2df01-888e-46c8-b17d-49fa3869b476", "uri": "../unitgroups/6ae2df01-888e-46c8-b17d-49fa3869b476.xml"}}, {"value": "4.8786035813269", "module": "A1"}, {"value": "0.00176984460596535", "module": "A2"}, {"value": "0.167359266003775", "module": "A3"}, {"value": "0", "module": "C1"}, {"value": "7.62844233005194E-05", "module": "C2"}, {"value": "0.5025843462612", "module": "C3"}, {"value": "1.62307791642724E-06", "module": "C4"}, {"value": "-0.269933996279825", "module": "D"}]}}, {"referenceToLCIAMethodDataSet": {"shortDescription": [{"value": "Incidence of disease due to PM emissions (PM)", "lang": "en"}, {"value": "Auftreten von Krankheiten aufgrund von Feinstaubemissionen (PM)", "lang": "de"}], "type": "LCIA method data set", "refObjectId": "b5c602c6-def3-11e6-bf01-fe55135034f3", "uri": "../lciamethods/b5c602c6-def3-11e6-bf01-fe55135034f3.xml"}, "other": {"anies": [{"name": "referenceToUnitGroupDataSet", "value": {"shortDescription": [{"value": "Disease incidence", "lang": "en"}], "type": "unit group data set", "refObjectId": "3883559b-648f-4afc-8ba2-0bd24f3affa3", "uri": "../unitgroups/3883559b-648f-4afc-8ba2-0bd24f3affa3.xml"}}, {"value": "66.6204635290747", "module": "A1"}, {"value": "3.94298823673184", "module": "A2"}, {"value": "9.60886179630474", "module": "A3"}, {"value": "0", "module": "C1"}, {"value": "0.0821189622117222", "module": "C2"}, {"value": "9.9893849749437", "module": "C3"}, {"value": "0.000107329452100118", "module": "C4"}, {"value": "-4.28529590113006", "module": "D"}]}}, {"referenceToLCIAMethodDataSet": {"shortDescription": [{"value": "Human exposure efficiency relative to U235 (IR)", "lang": "en"}, {"value": "Wirkung durch Exposition des Menschen mit U235 (IR)", "lang": "de"}], "type": "LCIA method data set", "refObjectId": "b5c632be-def3-11e6-bf01-fe55135034f3", "uri": "../lciamethods/b5c632be-def3-11e6-bf01-fe55135034f3.xml"}, "other": {"anies": [{"name": "referenceToUnitGroupDataSet", "value": {"shortDescription": [{"value": "kBq U235 eq", "lang": "en"}], "type": "unit group data set", "refObjectId": "456b05bf-1415-44a9-9993-02452f554c09", "uri": "../unitgroups/456b05bf-1415-44a9-9993-02452f554c09.xml"}}, {"value": "35.8058547730947", "module": "A1"}, {"value": "0.0693848591387284", "module": "A2"}, {"value": "24.0908279114427", "module": "A3"}, {"value": "0", "module": "C1"}, {"value": "0.00158964327238759", "module": "C2"}, {"value": "1.56760567426725", "module": "C3"}, {"value": "6.15027852904384E-06", "module": "C4"}, {"value": "-1.91304234381635", "module": "D"}]}}, {"referenceToLCIAMethodDataSet": {"shortDescription": [{"value": "Comparative toxic unit for ecosystems (ETP-fw)", "lang": "en"}, {"value": "Toxizitätsvergleichseinheit für Ökosysteme (ETP-fw)", "lang": "de"}], "type": "LCIA method data set", "refObjectId": "ee1082d1-b0f7-43ca-a1f0-21e2a4a74511", "uri": "../lciamethods/ee1082d1-b0f7-43ca-a1f0-21e2a4a74511.xml"}, "other": {"anies": [{"name": "referenceToUnitGroupDataSet", "value": {"shortDescription": [{"value": "CTUe", "lang": "en"}], "type": "unit group data set", "refObjectId": "aa959ded-f1eb-4efb-9c5c-2d60be36b3e6", "uri": "../unitgroups/aa959ded-f1eb-4efb-9c5c-2d60be36b3e6.xml"}}, {"value": "0.436464138551016", "module": "A1"}, {"value": "0.0357616437925614", "module": "A2"}, {"value": "0.0808452394478632", "module": "A3"}, {"value": "0", "module": "C1"}, {"value": "0.000789032502024501", "module": "C2"}, {"value": "0.0578967158112673", "module": "C3"}, {"value": "8.69460450524917E-07", "module": "C4"}, {"value": "-0.0431078680631369", "module": "D"}]}}, {"referenceToLCIAMethodDataSet": {"shortDescription": [{"value": "Comparative toxic unit for humans (carcinogenic) (HTP-c)", "lang": "en"}, {"value": "Toxizitätsvergleichseinheit für Menschen (krebserregend) (HTP-c)", "lang": "de"}], "type": "LCIA method data set", "refObjectId": "2299222a-bbd8-474f-9d4f-4dd1f18aea7c", "uri": "../lciamethods/2299222a-bbd8-474f-9d4f-4dd1f18aea7c.xml"}, "other": {"anies": [{"name": "referenceToUnitGroupDataSet", "value": {"shortDescription": [{"value": "CTUh", "lang": "en"}], "type": "unit group data set", "refObjectId": "d4c9523e-2d7e-49fd-8469-998f547d3a70", "uri": "../unitgroups/d4c9523e-2d7e-49fd-8469-998f547d3a70.xml"}}, {"value": "2.84988735051468E-19", "module": "A1"}, {"value": "1.32818023457577E-21", "module": "A2"}, {"value": "5.91297383813315E-20", "module": "A3"}, {"value": "0", "module": "C1"}, {"value": "2.93385853946133E-23", "module": "C2"}, {"value": "5.9232408900486E-20", "module": "C3"}, {"value": "1.84727885570744E-25", "module": "C4"}, {"value": "-2.53325588691882E-19", "module": "D"}]}}, {"referenceToLCIAMethodDataSet": {"shortDescription": [{"value": "Comparative toxic unit for humans (noncarcinogenic) (HTP-nc)", "lang": "en"}, {"value": "Toxizitätsvergleichseinheit für Menschen (nicht krebserregend) (HTP-nc)", "lang": "de"}], "type": "LCIA method data set", "refObjectId": "3af763a5-b7a1-48c9-9cee-1f223481fcef", "uri": "../lciamethods/3af763a5-b7a1-48c9-9cee-1f223481fcef.xml"}, "other": {"anies": [{"name": "referenceToUnitGroupDataSet", "value": {"shortDescription": [{"value": "CTUh", "lang": "en"}], "type": "unit group data set", "refObjectId": "d4c9523e-2d7e-49fd-8469-998f547d3a70", "uri": "../unitgroups/d4c9523e-2d7e-49fd-8469-998f547d3a70.xml"}}, {"value": "3.83165540302648E-09", "module": "A1"}, {"value": "7.59683100171706E-11", "module": "A2"}, {"value": "1.96144446101243E-10", "module": "A3"}, {"value": "0", "module": "C1"}, {"value": "1.66637042542256E-12", "module": "C2"}, {"value": "7.89297620365989E-10", "module": "C3"}, {"value": "1.63693222666336E-14", "module": "C4"}, {"value": "-8.91901084693888E-10", "module": "D"}]}}, {"referenceToLCIAMethodDataSet": {"shortDescription": [{"value": "Soil quality index (SQP)", "lang": "en"}, {"value": "Bodenqualitätsindex (SQP)", "lang": "de"}], "type": "LCIA method data set", "refObjectId": "b2ad6890-c78d-11e6-9d9d-cec0c932ce01", "uri": "../lciamethods/b2ad6890-c78d-11e6-9d9d-cec0c932ce01.xml"}, "other": {"anies": [{"name": "referenceToUnitGroupDataSet", "value": {"shortDescription": [{"value": "SQP", "lang": "en"}], "type": "unit group data set", "refObjectId": "f130951c-e67f-4f7f-8dd4-665de3974e18", "uri": "../unitgroups/f130951c-e67f-4f7f-8dd4-665de3974e18.xml"}}, {"value": "7.44983207012272E-08", "module": "A1"}, {"value": "1.71213089023738E-12", "module": "A2"}, {"value": "9.33089047707132E-11", "module": "A3"}, {"value": "0", "module": "C1"}, {"value": "3.89888635980712E-14", "module": "C2"}, {"value": "2.7431779174478E-11", "module": "C3"}, {"value": "4.93026365593758E-16", "module": "C4"}, {"value": "-3.85204873903725E-10", "module": "D"}]}}]}, "otherAttributes": {"{http://www.indata.network/EPD/2019}epd-version": "1.2"}, "version": "1.1", "locations": "../ILCDLocations.xml"}