{"processInformation": {"dataSetInformation": {"UUID": "231073e3-f6ab-44e1-8117-0d38b9c2e526", "name": {"baseName": [{"value": "Drawn Wire - Prestressing Wire and Strand", "lang": "en"}, {"value": "Spannstahl", "lang": "de"}], "functionalUnitFlowProperties": [{"lang": "en"}]}, "classificationInformation": {"classification": [{"class": [{"value": "Metalle", "level": 0, "classId": "4"}, {"value": "Stahl und Eisen", "level": 1, "classId": "4.1"}, {"value": "Stahlprofile", "level": 2, "classId": "4.1.03"}], "name": "OEKOBAU.DAT"}, {"class": [{"value": "02 Building products", "level": 0}, {"value": "Metallic products and ancillaries", "level": 1}, {"value": "Structural steels", "level": 2}], "name": "IBUCategories"}]}, "generalComment": [{"value": "Prestressing wires and strands are used for reinforcing concrete structures, such as large-span bridges, rock-soil anchoring solutions, multi-storey industrial buildings, stadiums, mines, sleepers etc. \n\nThe prestressing wires are produced according to FprEN 10138-2:2009 besides many other standards and homologations. Diameters range from 5.0 up to 10.5 mm.\n\nOur 7-wire prestressing strands are supplied with cross-sectional areas ranging from 139 to 165 mm, depending on customer requirements, and with smooth or compacted surface.\nCompacted prestressing strands have a cross-sectional area of 165 mm. All strands exhibit very low relaxation. They are produced according to FprEN 10138-3:2009 besides other standards and homologations. Diameters range from 15.2 to 15.7 mm for bare and compacted strands.\n\nvoestalpine Wire Technology also manufactures a variety of strand types with corrosion protection. The strands can be oiled, galvanized and additionally greased or waxed and PE-coated. Due to their excellent properties, these products are suitable for a wide variety of uses.\n\nThe prestressing products are manufactured under ideal processing conditions to ensure they meet the most demanding quality standards.\n\nContinuous quality inspections and many special testing options\nEnd-to-end traceability of all production and test parameters\nGreatest possible flexibility as the result of an integrated production chain\nStrict adherence to schedules, and partnerships with our customers\nTechnical and sales service", "lang": "en"}, {"value": "Spanndrähte und -litzen werden für die Verstärkung von Betonkonstruktionen verwendet, wie z.B. Brücken mit großer Spannweite, Fels-Boden-Verankerungen, mehrstöckige Industriegebäude, Stadien, Bergwerke, Schwellen usw. \n\nDie Spanndrähte werden gemäß FprEN 10138-2:2009 und vielen anderen Normen und Zulassungen hergestellt. Die Durchmesser reichen von 5,0 bis 10,5 mm. \n\nUnsere 7-drähtigen Spannlitzen werden je nach Kundenwunsch mit Querschnittsflächen von 139 bis 165 mm² und mit glatter oder verdichteter Oberfläche geliefert. Verdichtete Spannlitzen haben eine Querschnittsfläche von 165 mm². Alle Litzen weisen eine sehr geringe Relaxation auf. Sie werden nach FprEN 10138-3:2009 sowie nach anderen Normen und Zulassungen hergestellt. Die Durchmesser reichen von 15,2 bis 15,7 mm für blanke und verdichtete Litzen. \n\nvoestalpine Wire Technology stellt auch eine Reihe von Litzentypen mit Korrosionsschutz her. Die Litzen können geölt, verzinkt und zusätzlich gefettet oder gewachst und PE-beschichtet sein. Aufgrund ihrer hervorragenden Eigenschaften sind diese Produkte für eine Vielzahl von Anwendungen geeignet. \n\nDie Vorspannprodukte werden unter idealen Verarbeitungsbedingungen hergestellt, um sicherzustellen, dass sie höchsten Qualitätsansprüchen genügen. \nKontinuierliche Qualitätskontrollen und viele spezielle Prüfmöglichkeiten \nDurchgängige Rückverfolgbarkeit aller Produktions- und Prüfparameter \nGrößtmögliche Flexibilität durch eine integrierte Produktionskette \nStrikte Termintreue und Partnerschaft mit unseren Kunden \nTechnischer und vertrieblicher Service", "lang": "de"}]}, "quantitativeReference": {"referenceToReferenceFlow": [0]}, "time": {"referenceYear": 2023, "dataSetValidUntil": 2028, "other": {"anies": [{"name": "publicationDateOfEPD", "value": 1683590400000}]}}, "geography": {"locationOfOperationSupplyOrProduction": {"location": "AT"}}, "technology": {"technologyDescriptionAndIncludedProcesses": [{"value": "Manufacturing of prestressing strands The starting process is the pickling process. During pickling scale and rust from the surface of the wire rod coil are removed by dipping into hydrochloric acid. After several other treatments like phosphate coating and borax coating the wire rod coil is prepared for the next step cold drawing. On the drawing line, the single wire is drawn to the final diameter on a spool. Seven of these spools finally are lifted into the skip strander, where a seven-wire prestressing strand is produced. The main process during stranding is the thermomechanical treatment (pulling and heating = stabilizing) to finally get the special properties like low relaxation and good ductility on a high tensile level. In case of a galvanized strand the wire is pre-drawn and galvanized in our hot dip galvanizing line. After galvanizing the final drawing and the stranding remain the same. In case of HDPE-coated strands, the smooth, compacted or galvanized strands are greased or waxed and afterwards HDPE-coated in our extrusion line. We can produce the coated strands from coil to coil either as reelless coils or on wooden reels. Manufacturing of prestressing steel wires The starting process is the pickling process. During pickling scale and rust from the surface of the wire rod coil are removed by dipping into hydrochloric acid. After several other treatments like phosphate coating and borax coating the wire rod coil is prepared for the next step cold drawing. On the combined drawing and stabilizing line, the single wire is drawn to the final diameter either in coils or in bars. The main process during drawing is the thermomechanical treatment (pulling and heating = stabilizing) to finally get the special properties like low relaxation and good ductility on a high tensile level. The wires in coils are directly sent to final customers, the wires in bars can be additionally bent and threaded or just only threaded at the end of the bars. Thus, all different types of wires needed for sleeper production (bars, threaded bars, coils or threaded hairpins) can be provided. \nTechnical data: \nThe prestressing wires are produced according to FprEN 10138-2:2009 besides other standards and homologations. The technical data given for the products are generic literature data for steel as described e.g. in Key to Steel. No product specific test rules are applicable to the data given.\n\nDiameter and tensile strength class of Prestressing Wires:\n\n\nThe prestressing strands are produced according to FprEN 10138-3:2009 besides other standards and homologations.\n\nDiameter and tensile strength class of Prestressing Strands: \nDeclared unit: \nThis environmental product declaration refers to a declared unit of 1 tonne of average prestressing steel.", "lang": "en"}, {"value": "Herstellung von Vorspannlitzen\nDer erste Prozess ist das Beizen. Beim Beizen werden Zunder und Rost von der Oberfläche der Walzdrahtrolle durch Eintauchen in Salzsäure entfernt. Nach verschiedenen anderen Behandlungen wie Phosphatierung und Boraxbeschichtung wird die Walzdrahtrolle für den nächsten Schritt, das Kaltziehen, vorbereitet.\n\nAuf der Ziehlinie wird der einzelne Draht auf den endgültigen Durchmesser auf eine Spule gezogen. Sieben dieser Spulen werden schließlich in die Skipverseilmaschine gehoben, wo eine siebenadrige Vorspannlitze hergestellt wird. Der wichtigste Prozess beim Verseilen ist die thermomechanische Behandlung (Ziehen und Erhitzen = Stabilisieren), um schließlich die besonderen Eigenschaften wie geringe Relaxation und gute Dehnbarkeit auf hohem Zugniveau zu erhalten.\n\nIm Falle einer verzinkten Litze wird der Draht vorgezogen und in unserer Feuerverzinkungsanlage verzinkt. Nach der Verzinkung bleiben das endgültige Ziehen und die Verseilung gleich.\n\nBei HDPE-beschichteten Litzen werden die glatten, verdichteten oder verzinkten Litzen gefettet oder gewachst und anschließend in unserer Extrusionsanlage HDPE-beschichtet. Wir können die ummantelten Litzen von Coil zu Coil entweder als reelless Coils oder auf Holzspulen produzieren.  \n\nHerstellung von Spannstahldrähten\nDer erste Prozess ist das Beizen. Beim Beizen werden Zunder und Rost von der Oberfläche der Walzdrahtrolle durch Eintauchen in Salzsäure entfernt. Nach verschiedenen anderen Behandlungen wie Phosphatierung und Boraxbeschichtung wird die Walzdrahtrolle für den nächsten Schritt, das Kaltziehen, vorbereitet.\n\nAuf der kombinierten Zieh- und Stabilisierungsanlage wird der einzelne Draht entweder in Ringen oder in Stangen auf den endgültigen Durchmesser gezogen. Der wichtigste Prozess während des Ziehens ist die thermomechanische Behandlung (Ziehen und Erwärmen = Stabilisieren), um schließlich die besonderen Eigenschaften wie geringe Relaxation und gute Duktilität auf hohem Zugniveau zu erhalten.\n\nDie Drähte in Spulen werden direkt an die Endkunden versandt, die Drähte in Stäben können zusätzlich gebogen und mit Gewinde versehen werden oder nur am Ende der Stäbe mit Gewinde versehen werden. Somit können alle verschiedenen Arten von Drähten, die für die Schwellenproduktion benötigt werden (Stangen, Gewindestangen, Spulen oder Gewindehaarnadeln), geliefert werden. \nTechnische Daten: \nDie Spanndrähte werden gemäß FprEN 10138-2:2009 sowie anderen Normen und Zulassungen hergestellt. \n\nDie Spannlitzen werden gemäß FprEN 10138-3:2009 sowie anderen Normen und Zulassungen hergestellt.  \nDeklarierte Einheit: \nDiese Umweltproduktdeklaration bezieht sich auf eine deklarierte Einheit von 1 Tonne durchschnittlichen Spannstahl.", "lang": "de"}], "technologicalApplicability": [{"value": "Prestressing wires are mainly used for prestressing of concrete sleepers but can find their application also in prefabricated parts, beams, or reinforced tubes. Bare strands and PE-coated strands for prestressed concrete are suitable for large-span and large bays cast-in-place concrete floors, precast elements and beams and other special structures. As an additional application, these strands can be used in wind tower construction and anchoring systems. Galvanized and PE-coated strands mainly are used in stay-cable bridges.", "lang": "en"}, {"value": "Spanndrähte werden hauptsächlich zum Vorspannen von Betonschwellen verwendet, können aber auch in Fertigteilen, Trägern oder verstärkten Rohren zum Einsatz kommen. Blanke Litzen und PE-beschichtete Litzen für vorgespannten Beton eignen sich für Ortbetondecken mit großer Spannweite und großen Feldern, Fertigteile und Balken und andere Spezialkonstruktionen. Außerdem können diese Litzen beim Bau von Windtürmen und Verankerungssystemen eingesetzt werden. Verzinkte und PE-beschichtete Litzen werden hauptsächlich in Schrägseilbrücken verwendet.", "lang": "de"}], "referenceToTechnologyFlowDiagrammOrPicture": [{"shortDescription": [{"value": "Prestressing Table 1.png", "lang": "en"}], "type": "source data set", "refObjectId": "ba294752-d168-416f-b750-df2d8155da5c", "uri": "../sources/ba294752-d168-416f-b750-df2d8155da5c.xml"}, {"shortDescription": [{"value": "Prestressing Table 2.png", "lang": "en"}], "type": "source data set", "refObjectId": "a80a1a24-afde-4bb2-86b6-a10e43302fd3", "uri": "../sources/a80a1a24-afde-4bb2-86b6-a10e43302fd3.xml"}]}}, "modellingAndValidation": {"LCIMethodAndAllocation": {"typeOfDataSet": "EPD", "referenceToLCAMethodDetails": [{"shortDescription": [{"value": "Structural steels.pdf", "lang": "en"}], "type": "source data set", "refObjectId": "bfdc9cf7-a718-4579-a137-8387561070f2"}], "other": {"anies": [{"name": "subType", "value": "average dataset"}]}}, "dataSourcesTreatmentAndRepresentativeness": {"referenceToDataSource": [{"shortDescription": [{"value": "GaBi Database (all versions)", "lang": "en"}], "type": "source data set", "refObjectId": "28d74cc0-db8b-4d7e-bc44-5f6d56ce0c4a"}, {"shortDescription": [{"value": "GaBi Database Edition 2021, CUP 2021.01", "lang": "en"}], "type": "source data set", "refObjectId": "1cece811-7501-44d4-8067-9259bd5cb835"}], "useAdviceForDataSet": [{"value": "Scope: \nThis EPD is based on a declared unit of 1 metric tonne of average voestalpine prestressing steel produced at the production site in Bruck a.d. Mur (Austria). \nSystem boundary: \nThe life cycle assessment of average prestressing steel refers to a cradle-to-gate analysis with modules (A1–A3 + C +D). Subsequent life cycle phases are part of the analysis:\n\nModule A1–A3 | Production stage\nThe production stage includes the burdens of the production of prestressing steel of voestalpine Wire Austria GmbH at the production site in Bruck a.d. Mur. Most of the used steel wire is provided by the voestalpine Wire Rod Austria from St. Peter Freienstein. Thus, the upstream environmental impact of the steel supplied is represented by primary data of the respective production site. Material and energy flows for the pickling, drawing, cold rolling and galvanizing are considered. Electricity at Bruck a. d. Mur is provided from 100 % renewable energy (emission factor GWP-total: 14 g CO2-equivalents/kWh). Thermal energy provision is based on natural gas. Module A1–A3 also includes the production of the packaging.\n\nModule C1 | Deconstruction and demolition\nIt is assumed that the product is not connected with other materials and can therefore be dismantled. Associated efforts are negligible, no environmental impacts from the deconstruction of the products are declared.\n\nModule C2 | Transport \nThe transport to the disposal of the material is estimated declaring a 50 km radius to the waste processing.\n\nModule C3 | Waste processing \nProduct flows that reach Module D for recycling leave the product system in C3. Environmental impacts resulting from the grinding and sorting of steel scrap are not included due to the negligible expected environmental impact.\n\nModule C4 | Landfilling \nModule C4 declares the environmental impacts incurred by landfilling (5 % of the product).\n\nModule D | Benefits and loads beyond the system boundary\nThe potential for substituting primary steel with a recycling scenario (95 % of the product) is outlined in Module D.", "lang": "en"}, {"value": "Gültigkeitsbereich: \nDiese EPD basiert auf einer deklarierten Einheit von 1 Tonne durchschnittlichen voestalpine-Spannstahl, der am Produktionsstandort in Bruck a.d. Mur (Österreich) hergestellt wird. \nSystemgrenze: \nDie Ökobilanz des durchschnittlichen Spannstahls bezieht sich auf eine Cradle-to-Gate-Analyse mit den Modulen (A1-A3 + C +D). Nachfolgende Lebenszyklusphasen sind Teil der Analyse: \n\nModul A1-A3 | Produktionsstadium\nDas Produktionsstadium umfasst die Aufwendungen der Spannstahlproduktion der voestalpine Wire Austria GmbH am Produktionsstandort in Bruck a.d. Mur. Der Großteil des eingesetzten Stahldrahtes wird von der voestalpine Wire Rod Austria aus St. Peter Freienstein geliefert. Die vorgelagerten Umweltauswirkungen des gelieferten Stahls werden daher durch Primärdaten des jeweiligen Produktionsstandortes dargestellt. Material- und Energieströme für das Beizen, Ziehen, Kaltwalzen und Verzinken werden berücksichtigt. Die Stromversorgung in Bruck a. d. Mur erfolgt zu 100 % aus erneuerbaren Energien (Emissionsfaktor GWP-gesamt: 14 g CO2-Äquivalente/kWh). Die Bereitstellung von thermischer Energie erfolgt auf der Basis von Erdgas. Modul A1-A3 umfasst auch die Herstellung der Verpackung. \n\nModul C1 | Rückbau\nFür das End of Life Szenario wird angenommen, dass das Endprodukt nicht mit anderen Materialien verbunden ist und sortenrein rückgebaut werden kann. Die mit dem Rückbau\nverbundenen Aufwände werden damit als gering eingeschätzt und sind somit vernachlässigbar.\n\nModul C2 | Transport \nModul C2 beinhaltet den Transport zur Abfallbehandlung. Dazu wird der Transport via LKW über 50 km Transportdistanz als Szenario angesetzt\n\nModul C3 | Abfallbehandlung \nJener Produktfluss, der das Modul D zum Recycling erreicht, verlässt das Produktsystem in C3. Aufwendungen für die Zerkleinerung und Sortierung des Stahlschrottes sind aufgrund \nder Geringfügigkeit der zu erwartenden Umweltwirkung nicht enthalten.\n\nModul C4 | Entsorgung \nDas Modul C4 deklariert die durch die Deponierung (5 % des Produktes) entstehenden Umweltwirkungen.\n\nModul D | Nutzen und Lasten außerhalb der Systemgrenze \nIm Modul D werden die Substitutionspotenziale von Primärstahl durch ein Recyclingszenario (95 % des Produktes) dargestellt.", "lang": "de"}], "other": {"anies": [{"name": "referenceToOriginalEPD", "value": {"shortDescription": {"value": "Drawn Wire - Prestressing Wire and Strand.pdf", "defaultValue": "Drawn Wire - Prestressing Wire and Strand.pdf", "lstrings": [{"lang": "en", "value": "Drawn Wire - Prestressing Wire and Strand.pdf"}]}, "type": "source data set", "uuid": {"uuid": "ea34d5c5-fc16-49ec-9a42-2ce48bb6a7b9"}, "refObjectId": "ea34d5c5-fc16-49ec-9a42-2ce48bb6a7b9", "resourceURLs": ["https://oekobaudat.de/OEKOBAU.DAT/resource/sources/ea34d5c5-fc16-49ec-9a42-2ce48bb6a7b9/Drawn_Wire_-_Prestressing_Wire_and_Strand_18886.pdf?version=00.03.000"]}}]}}, "validation": {"review": [{"referenceToNameOfReviewerAndInstitution": [{"shortDescription": [{"value": "Institut Bauen und Umwelt e. V.", "lang": "en"}], "type": "contact data set", "refObjectId": "d111dbec-b024-4be5-86c5-752d6eb2cf95", "uri": "../contacts/d111dbec-b024-4be5-86c5-752d6eb2cf95.xml"}], "type": "Accredited third party review"}]}, "complianceDeclarations": {"compliance": [{"referenceToComplianceSystem": {"shortDescription": [{"value": "DIN EN 15804+A2", "lang": "en"}], "type": "source data set", "refObjectId": "c0016b33-8cf7-415c-ac6e-deba0d21440d", "uri": "../sources/c0016b33-8cf7-415c-ac6e-deba0d21440d.xml"}}, {"referenceToComplianceSystem": {"shortDescription": [{"value": "ISO 14025", "lang": "en"}], "type": "source data set", "refObjectId": "4f2eb655-6e44-4874-a95a-e28f5442cd4d", "uri": "../sources/4f2eb655-6e44-4874-a95a-e28f5442cd4d.xml"}}]}}, "administrativeInformation": {"commissionerAndGoal": {"referenceToCommissioner": [{"shortDescription": [{"value": "voestalpine AG", "lang": "en"}], "type": "contact data set", "refObjectId": "eef08a78-bb8b-429e-a968-c40f32a49ec7", "uri": "../contacts/eef08a78-bb8b-429e-a968-c40f32a49ec7.xml"}]}, "dataGenerator": {"referenceToPersonOrEntityGeneratingTheDataSet": [{"shortDescription": [{"value": "Daxner & Merl GmbH", "lang": "en"}], "type": "contact data set", "refObjectId": "ad8ad627-3991-42b7-a7ca-5a3fe0a34c28", "uri": "../contacts/ad8ad627-3991-42b7-a7ca-5a3fe0a34c28.xml"}]}, "dataEntryBy": {"timeStamp": 1683590400000, "referenceToDataSetFormat": [{"shortDescription": [{"value": "ILCD Format", "lang": "en"}], "type": "source data set", "refObjectId": "a97a0155-0234-4b87-b4ce-a45da52f2a40", "uri": "../sources/a97a0155-0234-4b87-b4ce-a45da52f2a40.xml"}, {"shortDescription": [{"value": "EPD-Datenformaterweiterungen v1.2", "lang": "de"}, {"value": "EPD Data Format Extensions v1.2", "lang": "en"}], "type": "source data set", "refObjectId": "a29449fd-aa2f-4de8-b5d7-4b06b43c6fde", "uri": "../sources/a29449fd-aa2f-4de8-b5d7-4b06b43c6fde.xml"}]}, "publicationAndOwnership": {"dataSetVersion": "00.06.100", "referenceToRegistrationAuthority": {"shortDescription": [{"value": "Institut Bauen und Umwelt e. V.", "lang": "en"}], "type": "contact data set", "refObjectId": "d111dbec-b024-4be5-86c5-752d6eb2cf95", "uri": "../contacts/d111dbec-b024-4be5-86c5-752d6eb2cf95.xml"}, "registrationNumber": "EPD-VOE-20230108-IBC2-EN", "referenceToOwnershipOfDataSet": {"shortDescription": [{"value": "voestalpine AG", "lang": "en"}], "type": "contact data set", "refObjectId": "eef08a78-bb8b-429e-a968-c40f32a49ec7", "uri": "../contacts/eef08a78-bb8b-429e-a968-c40f32a49ec7.xml"}, "copyright": true, "licenseType": "Free of charge for all users and uses", "accessRestrictions": [{"value": "None", "lang": "en"}], "other": {"anies": [{"name": "referenceToPublisher", "value": {"shortDescription": [{"value": "Institut Bauen und Umwelt e. V.", "lang": "en"}], "type": "contact data set", "refObjectId": "d111dbec-b024-4be5-86c5-752d6eb2cf95", "uri": "../contacts/d111dbec-b024-4be5-86c5-752d6eb2cf95.xml"}}]}}}, "exchanges": {"exchange": [{"dataSetInternalID": 0, "referenceToFlowDataSet": {"shortDescription": [{"value": "Spannstahl (Spannstahl)", "lang": "en"}], "type": "flow data set", "refObjectId": "ce2e0126-7d61-d131-6701-c9487823d5e0", "uri": "../flows/ce2e0126-7d61-d131-6701-c9487823d5e0.xml"}, "meanAmount": 1.0, "referencesToDataSource": {}, "referenceFlow": true, "resolvedFlowVersion": "00.01.100", "resultingflowAmount": 1000.0, "flowProperties": [{"name": [{"lang": "en", "value": "Mass"}, {"lang": "de", "value": "Masse"}], "uuid": "93a60a56-a3c8-11da-a746-0800200b9a66", "referenceFlowProperty": true, "meanValue": 1000.0, "referenceUnit": "kg", "unitGroupUUID": "ad38d542-3fe9-439d-9b95-2f5f7752acaf"}], "materialProperties": [{"name": "gross density", "value": "7850.0", "unit": "kg/m^3", "unitDescription": "kilograms per cubic metre"}], "typeOfFlow": "Product flow", "classification": {"classHierarchy": "Metalle / Stahl und Eisen / Stahlprofile", "name": "OEKOBAU.DAT"}}, {"dataSetInternalID": 1, "referenceToFlowDataSet": {"shortDescription": [{"value": "Renewable primary energy as energy carrier (PERE)", "lang": "en"}, {"value": "Erneuerbare Primärenergie als Energieträger (PERE)", "lang": "de"}], "type": "flow data set", "refObjectId": "20f32be5-0398-4288-9b6d-accddd195317", "uri": "../flows/20f32be5-0398-4288-9b6d-accddd195317.xml"}, "exchange direction": "INPUT", "other": {"anies": [{"name": "referenceToUnitGroupDataSet", "value": {"shortDescription": [{"value": "MJ", "lang": "en"}], "type": "unit group data set", "refObjectId": "93a60a57-a3c8-11da-a746-0800200c9a66", "uri": "../unitgroups/93a60a57-a3c8-11da-a746-0800200c9a66.xml"}}, {"value": "3192.54206977513", "module": "A1-A3"}, {"value": "0", "module": "C1"}, {"value": "2.29162705358998", "module": "C2"}, {"value": "0", "module": "C3"}, {"value": "2.56802636768431", "module": "C4"}, {"value": "1196.69855169921", "module": "D"}]}, "resolvedFlowVersion": "38.00.000", "flowProperties": [], "typeOfFlow": "Other flow", "classification": {"classHierarchy": "Quantities", "name": "GaBiCategories"}}, {"dataSetInternalID": 2, "referenceToFlowDataSet": {"shortDescription": [{"value": "Renewable primary energy resources as material utilization (PERM)", "lang": "en"}, {"value": "Erneuerbare Primärenergie zur stofflichen Nutzung (PERM)", "lang": "de"}], "type": "flow data set", "refObjectId": "fb3ec0de-548d-4508-aea5-00b73bf6f702", "uri": "../flows/fb3ec0de-548d-4508-aea5-00b73bf6f702.xml"}, "exchange direction": "INPUT", "other": {"anies": [{"name": "referenceToUnitGroupDataSet", "value": {"shortDescription": [{"value": "MJ", "lang": "en"}], "type": "unit group data set", "refObjectId": "93a60a57-a3c8-11da-a746-0800200c9a66", "uri": "../unitgroups/93a60a57-a3c8-11da-a746-0800200c9a66.xml"}}, {"value": "68.0731053858571", "module": "A1-A3"}, {"value": "0", "module": "C1"}, {"value": "0", "module": "C2"}, {"value": "0", "module": "C3"}, {"value": "0", "module": "C4"}, {"value": "0", "module": "D"}]}, "resolvedFlowVersion": "38.00.000", "flowProperties": [], "typeOfFlow": "Other flow", "classification": {"classHierarchy": "Quantities", "name": "GaBiCategories"}}, {"dataSetInternalID": 3, "referenceToFlowDataSet": {"shortDescription": [{"value": "Total use of renewable primary energy resources (PERT)", "lang": "en"}, {"value": "Total erneuerbare Primärenergie (PERT)", "lang": "de"}], "type": "flow data set", "refObjectId": "53f97275-fa8a-4cdd-9024-65936002acd0", "uri": "../flows/53f97275-fa8a-4cdd-9024-65936002acd0.xml"}, "exchange direction": "INPUT", "other": {"anies": [{"name": "referenceToUnitGroupDataSet", "value": {"shortDescription": [{"value": "MJ", "lang": "en"}], "type": "unit group data set", "refObjectId": "93a60a57-a3c8-11da-a746-0800200c9a66", "uri": "../unitgroups/93a60a57-a3c8-11da-a746-0800200c9a66.xml"}}, {"value": "3260.61517516099", "module": "A1-A3"}, {"value": "0", "module": "C1"}, {"value": "2.29162705358998", "module": "C2"}, {"value": "0", "module": "C3"}, {"value": "2.56802636768431", "module": "C4"}, {"value": "1196.69855169921", "module": "D"}]}, "resolvedFlowVersion": "38.00.000", "flowProperties": [], "typeOfFlow": "Other flow", "classification": {"classHierarchy": "Quantities / Environmental quantities / EPD EN 15804 / LCI indicators", "name": "GaBiCategories"}}, {"dataSetInternalID": 4, "referenceToFlowDataSet": {"shortDescription": [{"value": "Non renewable primary energy as energy carrier (PENRE)", "lang": "en"}, {"value": "Nicht-erneuerbare Primärenergie als Energieträger (PENRE)", "lang": "de"}], "type": "flow data set", "refObjectId": "ac857178-2b45-46ec-892a-a9a4332f0372", "uri": "../flows/ac857178-2b45-46ec-892a-a9a4332f0372.xml"}, "exchange direction": "INPUT", "other": {"anies": [{"name": "referenceToUnitGroupDataSet", "value": {"shortDescription": [{"value": "MJ", "lang": "en"}], "type": "unit group data set", "refObjectId": "93a60a57-a3c8-11da-a746-0800200c9a66", "uri": "../unitgroups/93a60a57-a3c8-11da-a746-0800200c9a66.xml"}}, {"value": "26355.0877869609", "module": "A1-A3"}, {"value": "0", "module": "C1"}, {"value": "39.9699776934577", "module": "C2"}, {"value": "0", "module": "C3"}, {"value": "35.560110058703", "module": "C4"}, {"value": "-13015.6390560097", "module": "D"}]}, "resolvedFlowVersion": "38.00.000", "flowProperties": [], "typeOfFlow": "Other flow", "classification": {"classHierarchy": "Quantities", "name": "GaBiCategories"}}, {"dataSetInternalID": 5, "referenceToFlowDataSet": {"shortDescription": [{"value": "Non renewable primary energy as material utilization (PENRM)", "lang": "en"}, {"value": "Nicht-erneuerbare Primärenergie zur stofflichen Nutzung (PENRM)", "lang": "de"}], "type": "flow data set", "refObjectId": "1421caa0-679d-4bf4-b282-0eb850ccae27", "uri": "../flows/1421caa0-679d-4bf4-b282-0eb850ccae27.xml"}, "exchange direction": "INPUT", "other": {"anies": [{"name": "referenceToUnitGroupDataSet", "value": {"shortDescription": [{"value": "MJ", "lang": "en"}], "type": "unit group data set", "refObjectId": "93a60a57-a3c8-11da-a746-0800200c9a66", "uri": "../unitgroups/93a60a57-a3c8-11da-a746-0800200c9a66.xml"}}, {"value": "1.161585724", "module": "A1-A3"}, {"value": "0", "module": "C1"}, {"value": "0", "module": "C2"}, {"value": "0", "module": "C3"}, {"value": "0", "module": "C4"}, {"value": "0", "module": "D"}]}, "resolvedFlowVersion": "38.00.000", "flowProperties": [], "typeOfFlow": "Other flow", "classification": {"classHierarchy": "Quantities", "name": "GaBiCategories"}}, {"dataSetInternalID": 6, "referenceToFlowDataSet": {"shortDescription": [{"value": "Total use of non renewable primary energy resources (PENRT)", "lang": "en"}, {"value": "Total nicht erneuerbare Primärenergie (PENRT)", "lang": "de"}], "type": "flow data set", "refObjectId": "06159210-646b-4c8d-8583-da9b3b95a6c1", "uri": "../flows/06159210-646b-4c8d-8583-da9b3b95a6c1.xml"}, "exchange direction": "INPUT", "other": {"anies": [{"name": "referenceToUnitGroupDataSet", "value": {"shortDescription": [{"value": "MJ", "lang": "en"}], "type": "unit group data set", "refObjectId": "93a60a57-a3c8-11da-a746-0800200c9a66", "uri": "../unitgroups/93a60a57-a3c8-11da-a746-0800200c9a66.xml"}}, {"value": "26356.2493726849", "module": "A1-A3"}, {"value": "0", "module": "C1"}, {"value": "39.9699776934577", "module": "C2"}, {"value": "0", "module": "C3"}, {"value": "35.560110058703", "module": "C4"}, {"value": "-13015.6390560097", "module": "D"}]}, "resolvedFlowVersion": "38.00.000", "flowProperties": [], "typeOfFlow": "Other flow", "classification": {"classHierarchy": "Quantities / Environmental quantities / EPD EN 15804 / LCI indicators", "name": "GaBiCategories"}}, {"dataSetInternalID": 7, "referenceToFlowDataSet": {"shortDescription": [{"value": "Use of secondary material (SM)", "lang": "en"}, {"value": "Einsatz von Sekundärstoffen (SM)", "lang": "de"}], "type": "flow data set", "refObjectId": "c6a1f35f-2d09-4f54-8dfb-97e502e1ce92", "uri": "../flows/c6a1f35f-2d09-4f54-8dfb-97e502e1ce92.xml"}, "exchange direction": "INPUT", "other": {"anies": [{"name": "referenceToUnitGroupDataSet", "value": {"shortDescription": [{"value": "kg", "lang": "en"}], "type": "unit group data set", "refObjectId": "ad38d542-3fe9-439d-9b95-2f5f7752acaf", "uri": "../unitgroups/ad38d542-3fe9-439d-9b95-2f5f7752acaf.xml"}}, {"value": "117.4398", "module": "A1-A3"}, {"value": "0", "module": "C1"}, {"value": "0", "module": "C2"}, {"value": "0", "module": "C3"}, {"value": "0", "module": "C4"}, {"value": "881.695", "module": "D"}]}, "resolvedFlowVersion": "38.00.000", "flowProperties": [], "typeOfFlow": "Other flow", "classification": {"classHierarchy": "Quantities / Environmental quantities / EPD EN 15804 / LCI indicators", "name": "GaBiCategories"}}, {"dataSetInternalID": 8, "referenceToFlowDataSet": {"shortDescription": [{"value": "Use of renewable secondary fuels (RSF)", "lang": "en"}, {"value": "Erneuerbare Sekundärbrennstoffe (RSF)", "lang": "de"}], "type": "flow data set", "refObjectId": "64333088-a55f-4aa2-9a31-c10b07816787", "uri": "../flows/64333088-a55f-4aa2-9a31-c10b07816787.xml"}, "exchange direction": "INPUT", "other": {"anies": [{"name": "referenceToUnitGroupDataSet", "value": {"shortDescription": [{"value": "MJ", "lang": "en"}], "type": "unit group data set", "refObjectId": "93a60a57-a3c8-11da-a746-0800200c9a66", "uri": "../unitgroups/93a60a57-a3c8-11da-a746-0800200c9a66.xml"}}, {"value": "0", "module": "A1-A3"}, {"value": "0", "module": "C1"}, {"value": "0", "module": "C2"}, {"value": "0", "module": "C3"}, {"value": "0", "module": "C4"}, {"value": "0", "module": "D"}]}, "resolvedFlowVersion": "38.00.000", "flowProperties": [], "typeOfFlow": "Other flow", "classification": {"classHierarchy": "Quantities / Environmental quantities / EPD EN 15804 / LCI indicators", "name": "GaBiCategories"}}, {"dataSetInternalID": 9, "referenceToFlowDataSet": {"shortDescription": [{"value": "Use of non renewable secondary fuels (NRSF)", "lang": "en"}, {"value": "Nicht erneuerbare Sekundärbrennstoffe (NRSF)", "lang": "de"}], "type": "flow data set", "refObjectId": "89def144-d39a-4287-b86f-efde453ddcb2", "uri": "../flows/89def144-d39a-4287-b86f-efde453ddcb2.xml"}, "exchange direction": "INPUT", "other": {"anies": [{"name": "referenceToUnitGroupDataSet", "value": {"shortDescription": [{"value": "MJ", "lang": "en"}], "type": "unit group data set", "refObjectId": "93a60a57-a3c8-11da-a746-0800200c9a66", "uri": "../unitgroups/93a60a57-a3c8-11da-a746-0800200c9a66.xml"}}, {"value": "0", "module": "A1-A3"}, {"value": "0", "module": "C1"}, {"value": "0", "module": "C2"}, {"value": "0", "module": "C3"}, {"value": "0", "module": "C4"}, {"value": "0", "module": "D"}]}, "resolvedFlowVersion": "38.00.000", "flowProperties": [], "typeOfFlow": "Other flow", "classification": {"classHierarchy": "Quantities / Environmental quantities / EPD EN 15804 / LCI indicators", "name": "GaBiCategories"}}, {"dataSetInternalID": 10, "referenceToFlowDataSet": {"shortDescription": [{"value": "Use of net fresh water (FW)", "lang": "en"}, {"value": "Einsatz von Süßwasserressourcen (FW)", "lang": "de"}], "type": "flow data set", "refObjectId": "3cf952c8-f3a4-461d-8c96-96456ca62246", "uri": "../flows/3cf952c8-f3a4-461d-8c96-96456ca62246.xml"}, "exchange direction": "INPUT", "other": {"anies": [{"name": "referenceToUnitGroupDataSet", "value": {"shortDescription": [{"value": "m^3", "lang": "en"}], "type": "unit group data set", "refObjectId": "cd950537-0a98-4044-9ba7-9f9a68d0a504", "uri": "../unitgroups/cd950537-0a98-4044-9ba7-9f9a68d0a504.xml"}}, {"value": "16.1930450845721", "module": "A1-A3"}, {"value": "0", "module": "C1"}, {"value": "0.00262465508256471", "module": "C2"}, {"value": "0", "module": "C3"}, {"value": "0.000367450889833254", "module": "C4"}, {"value": "-6.58801196784611", "module": "D"}]}, "resolvedFlowVersion": "38.00.000", "flowProperties": [], "typeOfFlow": "Other flow", "classification": {"classHierarchy": "Quantities / Environmental quantities / EPD EN 15804 / LCI indicators", "name": "GaBiCategories"}}, {"dataSetInternalID": 11, "referenceToFlowDataSet": {"shortDescription": [{"value": "Hazardous waste disposed (HWD)", "lang": "en"}, {"value": "Gefährlicher Abfall zur Deponie (HWD)", "lang": "de"}], "type": "flow data set", "refObjectId": "430f9e0f-59b2-46a0-8e0d-55e0e84948fc", "uri": "../flows/430f9e0f-59b2-46a0-8e0d-55e0e84948fc.xml"}, "exchange direction": "OUTPUT", "other": {"anies": [{"name": "referenceToUnitGroupDataSet", "value": {"shortDescription": [{"value": "kg", "lang": "en"}], "type": "unit group data set", "refObjectId": "ad38d542-3fe9-439d-9b95-2f5f7752acaf", "uri": "../unitgroups/ad38d542-3fe9-439d-9b95-2f5f7752acaf.xml"}}, {"value": "0.000391014352570897", "module": "A1-A3"}, {"value": "0", "module": "C1"}, {"value": "2.10610417494668E-09", "module": "C2"}, {"value": "0", "module": "C3"}, {"value": "6.30055255131535E-09", "module": "C4"}, {"value": "3.62936493839879E-06", "module": "D"}]}, "resolvedFlowVersion": "38.00.000", "flowProperties": [], "typeOfFlow": "Other flow", "classification": {"classHierarchy": "Quantities / Environmental quantities / EPD EN 15804 / LCI indicators", "name": "GaBiCategories"}}, {"dataSetInternalID": 12, "referenceToFlowDataSet": {"shortDescription": [{"value": "Non hazardous waste disposed (NHWD)", "lang": "en"}, {"value": "Entsorgter nicht gefährlicher Abfall (NHWD)", "lang": "de"}], "type": "flow data set", "refObjectId": "b29ef66b-e286-4afa-949f-62f1a7b4d7fa", "uri": "../flows/b29ef66b-e286-4afa-949f-62f1a7b4d7fa.xml"}, "exchange direction": "OUTPUT", "other": {"anies": [{"name": "referenceToUnitGroupDataSet", "value": {"shortDescription": [{"value": "kg", "lang": "en"}], "type": "unit group data set", "refObjectId": "ad38d542-3fe9-439d-9b95-2f5f7752acaf", "uri": "../unitgroups/ad38d542-3fe9-439d-9b95-2f5f7752acaf.xml"}}, {"value": "66.0089503817481", "module": "A1-A3"}, {"value": "0", "module": "C1"}, {"value": "0.006270810990958", "module": "C2"}, {"value": "0", "module": "C3"}, {"value": "50.0681660982345", "module": "C4"}, {"value": "156.454422959768", "module": "D"}]}, "resolvedFlowVersion": "38.00.000", "flowProperties": [], "typeOfFlow": "Other flow", "classification": {"classHierarchy": "Quantities / Environmental quantities / EPD EN 15804 / LCI indicators", "name": "GaBiCategories"}}, {"dataSetInternalID": 13, "referenceToFlowDataSet": {"shortDescription": [{"value": "Radioactive waste disposed (RWD)", "lang": "en"}, {"value": "Entsorgter radioaktiver Abfall (RWD)", "lang": "de"}], "type": "flow data set", "refObjectId": "3449546e-52ad-4b39-b809-9fb77cea8ff6", "uri": "../flows/3449546e-52ad-4b39-b809-9fb77cea8ff6.xml"}, "exchange direction": "OUTPUT", "other": {"anies": [{"name": "referenceToUnitGroupDataSet", "value": {"shortDescription": [{"value": "kg", "lang": "en"}], "type": "unit group data set", "refObjectId": "ad38d542-3fe9-439d-9b95-2f5f7752acaf", "uri": "../unitgroups/ad38d542-3fe9-439d-9b95-2f5f7752acaf.xml"}}, {"value": "0.120720449963045", "module": "A1-A3"}, {"value": "0", "module": "C1"}, {"value": "7.25025813208313E-05", "module": "C2"}, {"value": "0", "module": "C3"}, {"value": "0.00040531725055476", "module": "C4"}, {"value": "0.00047111142394864", "module": "D"}]}, "resolvedFlowVersion": "38.00.000", "flowProperties": [], "typeOfFlow": "Other flow", "classification": {"classHierarchy": "Quantities / Environmental quantities / EPD EN 15804 / LCI indicators", "name": "GaBiCategories"}}, {"dataSetInternalID": 14, "referenceToFlowDataSet": {"shortDescription": [{"value": "Components for re-use (CRU)", "lang": "en"}, {"value": "Komponenten für die Wiederverwendung (CRU)", "lang": "de"}], "type": "flow data set", "refObjectId": "a2b32f97-3fc7-4af2-b209-525bc6426f33", "uri": "../flows/a2b32f97-3fc7-4af2-b209-525bc6426f33.xml"}, "exchange direction": "OUTPUT", "other": {"anies": [{"name": "referenceToUnitGroupDataSet", "value": {"shortDescription": [{"value": "kg", "lang": "en"}], "type": "unit group data set", "refObjectId": "ad38d542-3fe9-439d-9b95-2f5f7752acaf", "uri": "../unitgroups/ad38d542-3fe9-439d-9b95-2f5f7752acaf.xml"}}, {"value": "0", "module": "A1-A3"}, {"value": "0", "module": "C1"}, {"value": "0", "module": "C2"}, {"value": "0", "module": "C3"}, {"value": "0", "module": "C4"}, {"value": "0", "module": "D"}]}, "resolvedFlowVersion": "38.00.000", "flowProperties": [], "typeOfFlow": "Other flow", "classification": {"classHierarchy": "Quantities / Environmental quantities / EPD EN 15804 / LCI indicators", "name": "GaBiCategories"}}, {"dataSetInternalID": 15, "referenceToFlowDataSet": {"shortDescription": [{"value": "Materials for recycling (MFR)", "lang": "en"}, {"value": "Stoffe zum Recycling (MFR)", "lang": "de"}], "type": "flow data set", "refObjectId": "d7fe48a5-4103-49c8-9aae-b0b5dfdbd6ae", "uri": "../flows/d7fe48a5-4103-49c8-9aae-b0b5dfdbd6ae.xml"}, "exchange direction": "OUTPUT", "other": {"anies": [{"name": "referenceToUnitGroupDataSet", "value": {"shortDescription": [{"value": "kg", "lang": "en"}], "type": "unit group data set", "refObjectId": "ad38d542-3fe9-439d-9b95-2f5f7752acaf", "uri": "../unitgroups/ad38d542-3fe9-439d-9b95-2f5f7752acaf.xml"}}, {"value": "0", "module": "A1-A3"}, {"value": "0", "module": "C1"}, {"value": "0", "module": "C2"}, {"value": "950", "module": "C3"}, {"value": "0", "module": "C4"}, {"value": "0", "module": "D"}]}, "resolvedFlowVersion": "38.00.000", "flowProperties": [], "typeOfFlow": "Other flow", "classification": {"classHierarchy": "Quantities / Environmental quantities / EPD EN 15804 / LCI indicators", "name": "GaBiCategories"}}, {"dataSetInternalID": 16, "referenceToFlowDataSet": {"shortDescription": [{"value": "Materials for energy recovery (MER)", "lang": "en"}, {"value": "Stoffe für die Energierückgewinnung (MER)", "lang": "de"}], "type": "flow data set", "refObjectId": "59a9181c-3aaf-46ee-8b13-2b3723b6e447", "uri": "../flows/59a9181c-3aaf-46ee-8b13-2b3723b6e447.xml"}, "exchange direction": "OUTPUT", "other": {"anies": [{"name": "referenceToUnitGroupDataSet", "value": {"shortDescription": [{"value": "kg", "lang": "en"}], "type": "unit group data set", "refObjectId": "ad38d542-3fe9-439d-9b95-2f5f7752acaf", "uri": "../unitgroups/ad38d542-3fe9-439d-9b95-2f5f7752acaf.xml"}}, {"value": "0", "module": "A1-A3"}, {"value": "0", "module": "C1"}, {"value": "0", "module": "C2"}, {"value": "0", "module": "C3"}, {"value": "0", "module": "C4"}, {"value": "0", "module": "D"}]}, "resolvedFlowVersion": "38.00.000", "flowProperties": [], "typeOfFlow": "Other flow", "classification": {"classHierarchy": "Quantities / Environmental quantities / EPD EN 15804 / LCI indicators", "name": "GaBiCategories"}}, {"dataSetInternalID": 17, "referenceToFlowDataSet": {"shortDescription": [{"value": "Exported electrical energy (EEE)", "lang": "en"}, {"value": "Exportierte elektrische Energie (EEE)", "lang": "de"}], "type": "flow data set", "refObjectId": "4da0c987-2b76-40d6-9e9e-82a017aaaf29", "uri": "../flows/4da0c987-2b76-40d6-9e9e-82a017aaaf29.xml"}, "exchange direction": "OUTPUT", "other": {"anies": [{"name": "referenceToUnitGroupDataSet", "value": {"shortDescription": [{"value": "MJ", "lang": "en"}], "type": "unit group data set", "refObjectId": "93a60a57-a3c8-11da-a746-0800200c9a66", "uri": "../unitgroups/93a60a57-a3c8-11da-a746-0800200c9a66.xml"}}, {"value": "0", "module": "A1-A3"}, {"value": "0", "module": "C1"}, {"value": "0", "module": "C2"}, {"value": "0", "module": "C3"}, {"value": "0", "module": "C4"}, {"value": "0", "module": "D"}]}, "resolvedFlowVersion": "38.00.000", "flowProperties": [], "typeOfFlow": "Other flow", "classification": {"classHierarchy": "Quantities / Environmental quantities / EPD EN 15804 / LCI indicators", "name": "GaBiCategories"}}, {"dataSetInternalID": 18, "referenceToFlowDataSet": {"shortDescription": [{"value": "Exported thermal energy (EET)", "lang": "en"}, {"value": "Exportierte thermische Energie (EET)", "lang": "de"}], "type": "flow data set", "refObjectId": "98daf38a-7a79-46d3-9a37-2b7bd0955810", "uri": "../flows/98daf38a-7a79-46d3-9a37-2b7bd0955810.xml"}, "exchange direction": "OUTPUT", "other": {"anies": [{"name": "referenceToUnitGroupDataSet", "value": {"shortDescription": [{"value": "MJ", "lang": "en"}], "type": "unit group data set", "refObjectId": "93a60a57-a3c8-11da-a746-0800200c9a66", "uri": "../unitgroups/93a60a57-a3c8-11da-a746-0800200c9a66.xml"}}, {"value": "0", "module": "A1-A3"}, {"value": "0", "module": "C1"}, {"value": "0", "module": "C2"}, {"value": "0", "module": "C3"}, {"value": "0", "module": "C4"}, {"value": "0", "module": "D"}]}, "resolvedFlowVersion": "38.00.000", "flowProperties": [], "typeOfFlow": "Other flow", "classification": {"classHierarchy": "Quantities / Environmental quantities / EPD EN 15804 / LCI indicators", "name": "GaBiCategories"}}]}, "LCIAResults": {"LCIAResult": [{"referenceToLCIAMethodDataSet": {"shortDescription": [{"value": "Global Warming Potential total (GWP-total)", "lang": "en"}, {"value": "Globales Erwärmungspotenzial total (GWP-total)", "lang": "de"}], "type": "LCIA method data set", "refObjectId": "6a37f984-a4b3-458a-a20a-64418c145fa2", "uri": "../lciamethods/6a37f984-a4b3-458a-a20a-64418c145fa2.xml"}, "other": {"anies": [{"name": "referenceToUnitGroupDataSet", "value": {"shortDescription": [{"value": "kg CO_(2) eq", "lang": "en"}], "type": "unit group data set", "refObjectId": "1ebf3012-d0db-4de2-aefd-ef30cedb0be1", "uri": "../unitgroups/1ebf3012-d0db-4de2-aefd-ef30cedb0be1.xml"}}, {"value": "2913.09726996597", "module": "A1-A3"}, {"value": "0", "module": "C1"}, {"value": "3.02406984359964", "module": "C2"}, {"value": "0", "module": "C3"}, {"value": "2.41918382472411", "module": "C4"}, {"value": "-1495.66416496684", "module": "D"}]}}, {"referenceToLCIAMethodDataSet": {"shortDescription": [{"value": "Global Warming Potential fossil fuels (GWP-fossil)", "lang": "en"}, {"value": "Globales Erwärmungspotenzial fossil (GWP-fossil)", "lang": "de"}], "type": "LCIA method data set", "refObjectId": "5f635281-343e-44fb-83df-1971b155e6b6", "uri": "../lciamethods/5f635281-343e-44fb-83df-1971b155e6b6.xml"}, "other": {"anies": [{"name": "referenceToUnitGroupDataSet", "value": {"shortDescription": [{"value": "kg CO_(2) eq", "lang": "en"}], "type": "unit group data set", "refObjectId": "1ebf3012-d0db-4de2-aefd-ef30cedb0be1", "uri": "../unitgroups/1ebf3012-d0db-4de2-aefd-ef30cedb0be1.xml"}}, {"value": "2895.55641373553", "module": "A1-A3"}, {"value": "0", "module": "C1"}, {"value": "3.00319194896064", "module": "C2"}, {"value": "0", "module": "C3"}, {"value": "2.44174990564248", "module": "C4"}, {"value": "-1494.91208396876", "module": "D"}]}}, {"referenceToLCIAMethodDataSet": {"shortDescription": [{"value": "Global Warming Potential biogenic (GWP-biogenic)", "lang": "en"}, {"value": "Globales Erwärmungspotenzial biogen (GWP-biogenic)", "lang": "de"}], "type": "LCIA method data set", "refObjectId": "2356e1ab-0185-4db5-86e5-16de51c7485c", "uri": "../lciamethods/2356e1ab-0185-4db5-86e5-16de51c7485c.xml"}, "other": {"anies": [{"name": "referenceToUnitGroupDataSet", "value": {"shortDescription": [{"value": "kg CO_(2) eq", "lang": "en"}], "type": "unit group data set", "refObjectId": "1ebf3012-d0db-4de2-aefd-ef30cedb0be1", "uri": "../unitgroups/1ebf3012-d0db-4de2-aefd-ef30cedb0be1.xml"}}, {"value": "16.4827449467717", "module": "A1-A3"}, {"value": "0", "module": "C1"}, {"value": "-0.00356121612494437", "module": "C2"}, {"value": "0", "module": "C3"}, {"value": "-0.0250097349651544", "module": "C4"}, {"value": "-0.968427013609688", "module": "D"}]}}, {"referenceToLCIAMethodDataSet": {"shortDescription": [{"value": "Global Warming Potential luluc (GWP-luluc)", "lang": "en"}, {"value": "Globales Erwärmungspotenzial luluc (GWP-luluc)", "lang": "de"}], "type": "LCIA method data set", "refObjectId": "4331bbdb-978a-490d-8707-eeb047f01a55", "uri": "../lciamethods/4331bbdb-978a-490d-8707-eeb047f01a55.xml"}, "other": {"anies": [{"name": "referenceToUnitGroupDataSet", "value": {"shortDescription": [{"value": "kg CO_(2) eq", "lang": "en"}], "type": "unit group data set", "refObjectId": "1ebf3012-d0db-4de2-aefd-ef30cedb0be1", "uri": "../unitgroups/1ebf3012-d0db-4de2-aefd-ef30cedb0be1.xml"}}, {"value": "1.05811128365918", "module": "A1-A3"}, {"value": "0", "module": "C1"}, {"value": "0.0244391107639501", "module": "C2"}, {"value": "0", "module": "C3"}, {"value": "0.0024436540467793", "module": "C4"}, {"value": "0.216346015532721", "module": "D"}]}}, {"referenceToLCIAMethodDataSet": {"shortDescription": [{"value": "Depletion potential of the stratospheric ozone layer (ODP)", "lang": "en"}, {"value": "Abbau Potential der stratosphärischen Ozonschicht (ODP)", "lang": "de"}], "type": "LCIA method data set", "refObjectId": "b5c629d6-def3-11e6-bf01-fe55135034f3", "uri": "../lciamethods/b5c629d6-def3-11e6-bf01-fe55135034f3.xml"}, "other": {"anies": [{"name": "referenceToUnitGroupDataSet", "value": {"shortDescription": [{"value": "kg CFC11 eq", "lang": "en"}], "type": "unit group data set", "refObjectId": "d9e957c9-7309-4474-bf3a-7777df6c4e5b", "uri": "../unitgroups/d9e957c9-7309-4474-bf3a-7777df6c4e5b.xml"}}, {"value": "2.18035141663722E-11", "module": "A1-A3"}, {"value": "0", "module": "C1"}, {"value": "5.90297134895215E-16", "module": "C2"}, {"value": "0", "module": "C3"}, {"value": "5.76801483752193E-15", "module": "C4"}, {"value": "-2.4925521788295E-12", "module": "D"}]}}, {"referenceToLCIAMethodDataSet": {"shortDescription": [{"value": "Acidification potential of land and water (AP)", "lang": "en"}, {"value": "Versauerungspotenzial von Boden und Wasser (AP)", "lang": "de"}], "type": "LCIA method data set", "refObjectId": "b5c611c6-def3-11e6-bf01-fe55135034f3", "uri": "../lciamethods/b5c611c6-def3-11e6-bf01-fe55135034f3.xml"}, "other": {"anies": [{"name": "referenceToUnitGroupDataSet", "value": {"shortDescription": [{"value": "mol H^(+) eq", "lang": "en"}], "type": "unit group data set", "refObjectId": "42e089ac-92bf-4bf2-8ca1-5fc40d18f2ed", "uri": "../unitgroups/42e089ac-92bf-4bf2-8ca1-5fc40d18f2ed.xml"}}, {"value": "9.09333594331628", "module": "A1-A3"}, {"value": "0", "module": "C1"}, {"value": "0.00991631767120497", "module": "C2"}, {"value": "0", "module": "C3"}, {"value": "0.00777562069923066", "module": "C4"}, {"value": "-2.68352411305563", "module": "D"}]}}, {"referenceToLCIAMethodDataSet": {"shortDescription": [{"value": "Eutrophication potential aquatic freshwater (EP-freshwater)", "lang": "en"}, {"value": "Eutrophierungspotenzial Süßwasser (EP-freshwater)", "lang": "de"}], "type": "LCIA method data set", "refObjectId": "b53ec18f-7377-4ad3-86eb-cc3f4f276b2b", "uri": "../lciamethods/b53ec18f-7377-4ad3-86eb-cc3f4f276b2b.xml"}, "other": {"anies": [{"name": "referenceToUnitGroupDataSet", "value": {"shortDescription": [{"value": "kg P eq", "lang": "en"}], "type": "unit group data set", "refObjectId": "0429039d-a61d-4590-ba67-aa4a20a810a1", "uri": "../unitgroups/0429039d-a61d-4590-ba67-aa4a20a810a1.xml"}}, {"value": "0.0151832512425223", "module": "A1-A3"}, {"value": "0", "module": "C1"}, {"value": "8.88275548806866E-06", "module": "C2"}, {"value": "0", "module": "C3"}, {"value": "1.8584714056159E-06", "module": "C4"}, {"value": "-0.00030568440945002", "module": "D"}]}}, {"referenceToLCIAMethodDataSet": {"shortDescription": [{"value": "Eutrophication potential aquatic marine (EP-marine)", "lang": "en"}, {"value": "Eutrophierungspotenzial Salzwasser (EP-marine)", "lang": "de"}], "type": "LCIA method data set", "refObjectId": "b5c619fa-def3-11e6-bf01-fe55135034f3", "uri": "../lciamethods/b5c619fa-def3-11e6-bf01-fe55135034f3.xml"}, "other": {"anies": [{"name": "referenceToUnitGroupDataSet", "value": {"shortDescription": [{"value": "kg N eq", "lang": "en"}], "type": "unit group data set", "refObjectId": "d05bb823-ecdf-4686-8c40-bf1d9257859f", "uri": "../unitgroups/d05bb823-ecdf-4686-8c40-bf1d9257859f.xml"}}, {"value": "2.18649721566573", "module": "A1-A3"}, {"value": "0", "module": "C1"}, {"value": "0.004554984082094", "module": "C2"}, {"value": "0", "module": "C3"}, {"value": "0.00193046056746469", "module": "C4"}, {"value": "-0.399931936093938", "module": "D"}]}}, {"referenceToLCIAMethodDataSet": {"shortDescription": [{"value": "Eutrophication potential terrestrial (EP-terrestrial)", "lang": "en"}, {"value": "Eutrophierungspotenzial Land (EP-terrestrial)", "lang": "de"}], "type": "LCIA method data set", "refObjectId": "b5c614d2-def3-11e6-bf01-fe55135034f3", "uri": "../lciamethods/b5c614d2-def3-11e6-bf01-fe55135034f3.xml"}, "other": {"anies": [{"name": "referenceToUnitGroupDataSet", "value": {"shortDescription": [{"value": "mol N eq", "lang": "en"}], "type": "unit group data set", "refObjectId": "71b4d617-0ec9-4d3f-b65e-e438940c2401", "uri": "../unitgroups/71b4d617-0ec9-4d3f-b65e-e438940c2401.xml"}}, {"value": "23.3379072901597", "module": "A1-A3"}, {"value": "0", "module": "C1"}, {"value": "0.0508448603038948", "module": "C2"}, {"value": "0", "module": "C3"}, {"value": "0.0211802245417931", "module": "C4"}, {"value": "-3.89896734375629", "module": "D"}]}}, {"referenceToLCIAMethodDataSet": {"shortDescription": [{"value": "Formation potential of tropospheric ozone photochemical oxidants (POCP)", "lang": "en"}, {"value": "Bildungspotential für troposphärisches Ozon (POCP)", "lang": "de"}], "type": "LCIA method data set", "refObjectId": "b5c610fe-def3-11e6-bf01-fe55135034f3", "uri": "../lciamethods/b5c610fe-def3-11e6-bf01-fe55135034f3.xml"}, "other": {"anies": [{"name": "referenceToUnitGroupDataSet", "value": {"shortDescription": [{"value": "kg NMVOC eq", "lang": "en"}], "type": "unit group data set", "refObjectId": "d27c25f8-fbc1-44c6-b47b-4adbae4199c6", "uri": "../unitgroups/d27c25f8-fbc1-44c6-b47b-4adbae4199c6.xml"}}, {"value": "7.30903113514778", "module": "A1-A3"}, {"value": "0", "module": "C1"}, {"value": "0.0089410805422895", "module": "C2"}, {"value": "0", "module": "C3"}, {"value": "0.00608284454471822", "module": "C4"}, {"value": "-2.04751058249074", "module": "D"}]}}, {"referenceToLCIAMethodDataSet": {"shortDescription": [{"value": "Abiotic depletion potential for non fossil resources (ADPE)", "lang": "en"}, {"value": "Potenzial für den abiotischen Abbau nicht fossiler Ressourcen (ADPE)", "lang": "de"}], "type": "LCIA method data set", "refObjectId": "b2ad6494-c78d-11e6-9d9d-cec0c932ce01", "uri": "../lciamethods/b2ad6494-c78d-11e6-9d9d-cec0c932ce01.xml"}, "other": {"anies": [{"name": "referenceToUnitGroupDataSet", "value": {"shortDescription": [{"value": "kg Sb eq", "lang": "en"}], "type": "unit group data set", "refObjectId": "54ccd2d9-a32a-4fc2-923d-f2c8c93e89d4", "uri": "../unitgroups/54ccd2d9-a32a-4fc2-923d-f2c8c93e89d4.xml"}}, {"value": "0.00457899723089705", "module": "A1-A3"}, {"value": "0", "module": "C1"}, {"value": "2.65013565513285E-07", "module": "C2"}, {"value": "0", "module": "C3"}, {"value": "1.68496269109713E-07", "module": "C4"}, {"value": "-0.00325269954443088", "module": "D"}]}}, {"referenceToLCIAMethodDataSet": {"shortDescription": [{"value": "Abiotic depletion potential for fossil resources (ADPF)", "lang": "en"}, {"value": "Potenzial für den abiotischen Abbau fossiler Brennstoffe (ADPF)", "lang": "de"}], "type": "LCIA method data set", "refObjectId": "b2ad6110-c78d-11e6-9d9d-cec0c932ce01", "uri": "../lciamethods/b2ad6110-c78d-11e6-9d9d-cec0c932ce01.xml"}, "other": {"anies": [{"name": "referenceToUnitGroupDataSet", "value": {"shortDescription": [{"value": "MJ", "lang": "en"}], "type": "unit group data set", "refObjectId": "93a60a57-a3c8-11da-a746-0800200c9a66", "uri": "../unitgroups/93a60a57-a3c8-11da-a746-0800200c9a66.xml"}}, {"value": "26267.2958198827", "module": "A1-A3"}, {"value": "0", "module": "C1"}, {"value": "39.8249241581825", "module": "C2"}, {"value": "0", "module": "C3"}, {"value": "35.5528764029718", "module": "C4"}, {"value": "-13011.7002563165", "module": "D"}]}}, {"referenceToLCIAMethodDataSet": {"shortDescription": [{"value": "Water use (WDP)", "lang": "en"}, {"value": "Wassernutzung (WDP)", "lang": "de"}], "type": "LCIA method data set", "refObjectId": "b2ad66ce-c78d-11e6-9d9d-cec0c932ce01", "uri": "../lciamethods/b2ad66ce-c78d-11e6-9d9d-cec0c932ce01.xml"}, "other": {"anies": [{"name": "referenceToUnitGroupDataSet", "value": {"shortDescription": [{"value": "m^(3) world eq deprived", "lang": "en"}], "type": "unit group data set", "refObjectId": "6ae2df01-888e-46c8-b17d-49fa3869b476", "uri": "../unitgroups/6ae2df01-888e-46c8-b17d-49fa3869b476.xml"}}, {"value": "523.450366008969", "module": "A1-A3"}, {"value": "0", "module": "C1"}, {"value": "0.0277457256015725", "module": "C2"}, {"value": "0", "module": "C3"}, {"value": "-0.0289389620167935", "module": "C4"}, {"value": "-293.350454773566", "module": "D"}]}}, {"referenceToLCIAMethodDataSet": {"shortDescription": [{"value": "Incidence of disease due to PM emissions (PM)", "lang": "en"}, {"value": "Auftreten von Krankheiten aufgrund von Feinstaubemissionen (PM)", "lang": "de"}], "type": "LCIA method data set", "refObjectId": "b5c602c6-def3-11e6-bf01-fe55135034f3", "uri": "../lciamethods/b5c602c6-def3-11e6-bf01-fe55135034f3.xml"}, "other": {"anies": [{"name": "referenceToUnitGroupDataSet", "value": {"shortDescription": [{"value": "Disease incidence", "lang": "en"}], "type": "unit group data set", "refObjectId": "3883559b-648f-4afc-8ba2-0bd24f3affa3", "uri": "../unitgroups/3883559b-648f-4afc-8ba2-0bd24f3affa3.xml"}}, {"module": "A1-A3"}, {"module": "C1"}, {"module": "C2"}, {"module": "C3"}, {"module": "C4"}, {"module": "D"}]}}, {"referenceToLCIAMethodDataSet": {"shortDescription": [{"value": "Human exposure efficiency relative to U235 (IR)", "lang": "en"}, {"value": "Wirkung durch Exposition des Menschen mit U235 (IR)", "lang": "de"}], "type": "LCIA method data set", "refObjectId": "b5c632be-def3-11e6-bf01-fe55135034f3", "uri": "../lciamethods/b5c632be-def3-11e6-bf01-fe55135034f3.xml"}, "other": {"anies": [{"name": "referenceToUnitGroupDataSet", "value": {"shortDescription": [{"value": "kBq U235 eq", "lang": "en"}], "type": "unit group data set", "refObjectId": "456b05bf-1415-44a9-9993-02452f554c09", "uri": "../unitgroups/456b05bf-1415-44a9-9993-02452f554c09.xml"}}, {"module": "A1-A3"}, {"module": "C1"}, {"module": "C2"}, {"module": "C3"}, {"module": "C4"}, {"module": "D"}]}}, {"referenceToLCIAMethodDataSet": {"shortDescription": [{"value": "Comparative toxic unit for ecosystems (ETP-fw)", "lang": "en"}, {"value": "Toxizitätsvergleichseinheit für Ökosysteme (ETP-fw)", "lang": "de"}], "type": "LCIA method data set", "refObjectId": "ee1082d1-b0f7-43ca-a1f0-21e2a4a74511", "uri": "../lciamethods/ee1082d1-b0f7-43ca-a1f0-21e2a4a74511.xml"}, "other": {"anies": [{"name": "referenceToUnitGroupDataSet", "value": {"shortDescription": [{"value": "CTUe", "lang": "en"}], "type": "unit group data set", "refObjectId": "aa959ded-f1eb-4efb-9c5c-2d60be36b3e6", "uri": "../unitgroups/aa959ded-f1eb-4efb-9c5c-2d60be36b3e6.xml"}}, {"module": "A1-A3"}, {"module": "C1"}, {"module": "C2"}, {"module": "C3"}, {"module": "C4"}, {"module": "D"}]}}, {"referenceToLCIAMethodDataSet": {"shortDescription": [{"value": "Comparative toxic unit for humans (carcinogenic) (HTP-c)", "lang": "en"}, {"value": "Toxizitätsvergleichseinheit für Menschen (krebserregend) (HTP-c)", "lang": "de"}], "type": "LCIA method data set", "refObjectId": "2299222a-bbd8-474f-9d4f-4dd1f18aea7c", "uri": "../lciamethods/2299222a-bbd8-474f-9d4f-4dd1f18aea7c.xml"}, "other": {"anies": [{"name": "referenceToUnitGroupDataSet", "value": {"shortDescription": [{"value": "CTUh", "lang": "en"}], "type": "unit group data set", "refObjectId": "d4c9523e-2d7e-49fd-8469-998f547d3a70", "uri": "../unitgroups/d4c9523e-2d7e-49fd-8469-998f547d3a70.xml"}}, {"module": "A1-A3"}, {"module": "C1"}, {"module": "C2"}, {"module": "C3"}, {"module": "C4"}, {"module": "D"}]}}, {"referenceToLCIAMethodDataSet": {"shortDescription": [{"value": "Comparative toxic unit for humans (noncarcinogenic) (HTP-nc)", "lang": "en"}, {"value": "Toxizitätsvergleichseinheit für Menschen (nicht krebserregend) (HTP-nc)", "lang": "de"}], "type": "LCIA method data set", "refObjectId": "3af763a5-b7a1-48c9-9cee-1f223481fcef", "uri": "../lciamethods/3af763a5-b7a1-48c9-9cee-1f223481fcef.xml"}, "other": {"anies": [{"name": "referenceToUnitGroupDataSet", "value": {"shortDescription": [{"value": "CTUh", "lang": "en"}], "type": "unit group data set", "refObjectId": "d4c9523e-2d7e-49fd-8469-998f547d3a70", "uri": "../unitgroups/d4c9523e-2d7e-49fd-8469-998f547d3a70.xml"}}, {"module": "A1-A3"}, {"module": "C1"}, {"module": "C2"}, {"module": "C3"}, {"module": "C4"}, {"module": "D"}]}}, {"referenceToLCIAMethodDataSet": {"shortDescription": [{"value": "Soil quality index (SQP)", "lang": "en"}, {"value": "Bodenqualitätsindex (SQP)", "lang": "de"}], "type": "LCIA method data set", "refObjectId": "b2ad6890-c78d-11e6-9d9d-cec0c932ce01", "uri": "../lciamethods/b2ad6890-c78d-11e6-9d9d-cec0c932ce01.xml"}, "other": {"anies": [{"name": "referenceToUnitGroupDataSet", "value": {"shortDescription": [{"value": "SQP", "lang": "en"}], "type": "unit group data set", "refObjectId": "f130951c-e67f-4f7f-8dd4-665de3974e18", "uri": "../unitgroups/f130951c-e67f-4f7f-8dd4-665de3974e18.xml"}}, {"module": "A1-A3"}, {"module": "C1"}, {"module": "C2"}, {"module": "C3"}, {"module": "C4"}, {"module": "D"}]}}]}, "otherAttributes": {"{http://www.indata.network/EPD/2019}epd-version": "1.2"}, "version": "1.1", "locations": "../ILCDLocations.xml"}