{"processInformation": {"dataSetInformation": {"UUID": "24a1470f-b2fd-4c55-9e3a-500e73041319", "name": {"baseName": [{"value": "Modulares Glasdach MS78", "lang": "en"}]}, "classificationInformation": {"classification": [{"class": [{"value": "Komponenten von Fenstern und Vorhangfassaden", "level": 0, "classId": "7"}, {"value": "Fenster", "level": 1, "classId": "7.8"}, {"value": "Sonstige Fenster", "level": 2, "classId": "7.8.05"}], "name": "OEKOBAU.DAT"}]}, "generalComment": [{"value": "The owner of this EPD shall be liable for the underlying information and evidence. The programme operator Kiwa-Ecobility Experts shall not be liable with respect to manufacturer data, life cycle assessment data and evidence.", "lang": "en"}], "other": {"anies": [{"scenario": [{"description": [{"value": "The Modulares Glasdach MS78 can be freely configurated in width and height so that it can be customised to the customers' requirements. For this EPD, the Modulares Glasdach MS78 with 2 modules that both have a width of 1,00 m and a height of 0,90 m have been selected. This product has a surface area of 1,82 m², but since the functional unit should be 1 m² according to the PCR, all inputs have been recalculated to 1 m². The results can be calculated for the full Modulares Glasdach MS78 of 1,82 m² by multiplying the results by 1,82. For this product, several raw materials are used that consist of secondary material, sometimes having a mixture of primary and secondary material. This has been reflected accurately in the LCA, and proof has been provided on the secondary content of the respective materials. For module A4 (transportation to the customer or construction site), both customers inside and outside Germany were taken into account. In 2022, 72,7% of revenue is attributable to domestic sales (i.e. within Germany) and 27,3% to international sales. This was taken into account when calculating the transportation distance for module A4. Transportation to domestic customers is carried out in small batches via distributors and consists of 2 parts, namely a longer route with a large truck (40 t) and a shorter route with a smaller truck (7.5 t). Here, a deviation has been made from the PCR (DIN EN 17213), because an internal calculation could be made.  How the MS78 modular glass roof is assembled and disassembled depends largely on the customer. As it is a large product with glass, this LCA assumes that the product must be installed and dismantled using a crane. Therefore, the electricity consumption for modules A5 (assembly) and C1 (disassembly) was taken into account. The electricity consumption for this crane was calculated in kWh per m² and the environmental profile of the European electricity standard (low voltage) was applied to take account of Lamilux's international clientele. The same scenario was assumed for modules A5 and C1. The scenarios modelled for these modules are currently in use and are representative for the most likely scenarios."}], "name": "Standard scenario", "default": true}]}]}}, "quantitativeReference": {"referenceToReferenceFlow": [1], "type": "Reference flow(s)"}, "time": {"referenceYear": 2024, "dataSetValidUntil": 2029, "timeRepresentativenessDescription": [{"value": "The data was collected in the beginning of 2024.", "lang": "en"}], "other": {"anies": [{"name": "publicationDateOfEPD", "value": 1718236800000}]}}, "geography": {"locationOfOperationSupplyOrProduction": {"descriptionOfRestrictions": [{"value": "The data are representative for Germany.", "lang": "en"}], "location": "DE"}}, "technology": {"technologyDescriptionAndIncludedProcesses": [{"value": "The Modulares Glasdach MS78 is a daylight element. It is available in widths of up to 3 meters with variable lengths. It can be installed with an inclination of between 5° and 30°. This, together with the flat glass surface and the frame profile on the eaves side, ensures optimum water drainage. Dirt edges are also avoided and the glass surfaces are cleaner. The high glass proportion of the MS78 provides an optimal daylight incidence. The MS78 also allows a custom integration of vents, ensuring a maximum supply of fresh air to a building. It guarantees maximum safety from the first sealing level thanks to a butt-jointed drainage profile (SEP), the best quality standards thanks to a high degree of prefabrication as well as durable and easy-to-clean materials and surfaces. The product is produced in Germany, and sold both inside and outside of Germany. The Modulares Glasdach MS78 is manufactured in three different steps. First, the raw materials are supplied. Then the sheet metal is laser cut and bent. Then there are three different production processes. The first is the production of the base frames. Then the fixed/sash frames are produced. Finally, the weather sheets are produced. Each of these three elements is transported to the construction site and assembled there.", "lang": "en"}], "technologicalApplicability": [{"value": "The Modulares Glasdach MS78 can be used on roofs to provide daylight and ventilate a building.", "lang": "en"}], "referenceToTechnologyFlowDiagrammOrPicture": [{"shortDescription": [{"value": "Flow chart Modulares Glasdach MS78", "lang": "en"}], "type": "source data set", "refObjectId": "17811e29-4eeb-4cef-9755-bb168c62ee5c", "version": "00.00.001"}]}}, "modellingAndValidation": {"LCIMethodAndAllocation": {"typeOfDataSet": "EPD", "other": {"anies": [{"name": "subType", "value": "specific dataset"}]}}, "dataSourcesTreatmentAndRepresentativeness": {"referenceToDataSource": [{"shortDescription": [{"value": "ecoinvent 3.6 database", "lang": "en"}], "type": "source data set", "refObjectId": "766b9973-5ee8-48a2-8098-72c8e20b369f", "version": "00.00.001"}, {"shortDescription": [{"value": "ecoinvent database (general)", "lang": "en"}], "type": "source data set", "refObjectId": "b497a91f-e14b-4b69-8f28-f50eb1576766", "version": "00.03.002"}], "useAdviceForDataSet": [{"value": "The Modulares Glasdach MS78 can be used on roofs to provide daylight and ventilate a building.", "lang": "en"}], "other": {"anies": [{"name": "referenceToOriginalEPD", "value": {"shortDescription": {"value": "Modulares Glasdach MS78 EPD", "defaultValue": "Modulares Glasdach MS78 EPD", "lstrings": [{"lang": "en", "value": "Modulares Glasdach MS78 EPD"}]}, "version": {"version": 1, "majorVersion": 0, "minorVersion": 0, "subMinorVersion": 1, "zero": false, "versionString": "00.00.001"}, "type": "source data set", "uuid": {"uuid": "0f952189-bf88-4b70-a086-1bcda97a9c09"}, "refObjectId": "0f952189-bf88-4b70-a086-1bcda97a9c09", "versionAsString": "00.00.001", "resourceURLs": ["https://oekobaudat.de/OEKOBAU.DAT/resource/sources/0f952189-bf88-4b70-a086-1bcda97a9c09/EPD-Kiwa-EE-167790-EN.pdf?version=00.00.001"]}}]}}, "validation": {"review": [{"reviewDetails": [{"value": "The independent verification is in accordance with the ISO 14025:2011.", "lang": "en"}], "referenceToNameOfReviewerAndInstitution": [{"shortDescription": [{"value": "Lucas Pedro Berman, Senda", "lang": "en"}], "type": "contact data set", "refObjectId": "2294137c-5a52-4a75-965f-770e74b24b10", "version": "00.00.002"}], "type": "Independent external review"}]}, "complianceDeclarations": {"compliance": [{"referenceToComplianceSystem": {"shortDescription": [{"value": "ISO 14025", "lang": "en"}], "type": "source data set", "refObjectId": "4f2eb655-6e44-4874-a95a-e28f5442cd4d", "version": "00.00.001"}}, {"referenceToComplianceSystem": {"shortDescription": [{"value": "EN 15804+A2", "lang": "de"}, {"value": "EN 15804+A2", "lang": "en"}], "type": "source data set", "refObjectId": "c0016b33-8cf7-415c-ac6e-deba0d21440d", "version": "00.01.000"}}]}}, "administrativeInformation": {"commissionerAndGoal": {"referenceToCommissioner": [{"shortDescription": [{"value": "LAMILUX Heinrich Strunz GmbH", "lang": "en"}], "type": "contact data set", "refObjectId": "861dae74-78e6-420e-ba2d-1ea91aaf5147", "version": "00.00.001"}]}, "dataGenerator": {"referenceToPersonOrEntityGeneratingTheDataSet": [{"shortDescription": [{"value": "Kiwa GmbH (Berlin)", "lang": "en"}], "type": "contact data set", "refObjectId": "3ea4a87a-3f88-4633-b7e7-1bbdd272be43", "version": "00.00.002"}]}, "dataEntryBy": {"timeStamp": 1728470008358, "referenceToDataSetFormat": [{"shortDescription": [{"value": "EPD Data Format Extensions v1.2", "lang": "en"}, {"value": "EPD-Datenformaterweiterungen v1.2", "lang": "de"}], "type": "source data set", "refObjectId": "a29449fd-aa2f-4de8-b5d7-4b06b43c6fde", "version": "00.01.000"}, {"shortDescription": [{"value": "ILCD format", "lang": "en"}], "type": "source data set", "refObjectId": "a97a0155-0234-4b87-b4ce-a45da52f2a40", "version": "01.00.001", "uri": "http://lca.jrc.ec.europa.eu/lcainfohub/sample_data/ilcd/sources/ILCD_Format_a97a0155-0234-4b87-b4ce-a45da52f2a40_01.00.000.xml"}], "referenceToPersonOrEntityEnteringTheData": {"shortDescription": [{"value": "Kiwa GmbH (Berlin)", "lang": "en"}], "type": "contact data set", "refObjectId": "3ea4a87a-3f88-4633-b7e7-1bbdd272be43", "version": "00.00.002"}}, "publicationAndOwnership": {"dataSetVersion": "00.00.007", "referenceToRegistrationAuthority": {"shortDescription": [{"value": "Kiwa-Ecobility Experts, Kiwa GmbH (Berlin)", "lang": "en"}], "type": "contact data set", "refObjectId": "eb52a9a8-9d0f-40ce-a5c9-7b78f5615e5a", "version": "00.00.002"}, "registrationNumber": "EPD-Kiwa-EE-167790-EN", "referenceToOwnershipOfDataSet": {"shortDescription": [{"value": "LAMILUX Heinrich Strunz GmbH", "lang": "en"}], "type": "contact data set", "refObjectId": "861dae74-78e6-420e-ba2d-1ea91aaf5147", "version": "00.00.001"}, "copyright": true, "licenseType": "Free of charge for all users and uses", "accessRestrictions": [{"value": "None.", "lang": "en"}], "other": {"anies": [{"name": "referenceToPublisher", "value": {"shortDescription": [{"value": "Kiwa-Ecobility Experts, Kiwa GmbH (Berlin)", "lang": "en"}], "type": "contact data set", "refObjectId": "eb52a9a8-9d0f-40ce-a5c9-7b78f5615e5a", "version": "00.00.002"}}]}}}, "exchanges": {"exchange": [{"dataSetInternalID": 1, "referenceToFlowDataSet": {"shortDescription": [{"value": "Modulares Glasdach MS78", "lang": "en"}], "type": "flow data set", "refObjectId": "b7030fad-4333-4377-ab2d-b45e565d744d", "version": "00.00.001"}, "meanAmount": 1.0, "resultingAmount": 1.0, "referenceFlow": true, "resultingflowAmount": 1.0, "flowProperties": [{"name": [{"lang": "de", "value": "Fläche"}, {"lang": "en", "value": "Area"}], "uuid": "93a60a56-a3c8-19da-a746-0800200c9a66", "referenceFlowProperty": true, "meanValue": 1.0, "referenceUnit": "qm", "unitGroupUUID": "c20a03d7-bd90-4569-bc94-66cfd364dfc8"}], "materialProperties": [{"name": "grammage", "value": "87.455", "unit": "kg/m^2", "unitDescription": "kilograms per square meter"}, {"name": "layer thickness", "value": "0.43", "unit": "m", "unitDescription": "meters"}], "typeOfFlow": "Product flow", "classification": {"classHierarchy": "Komponenten von Fenstern und Vorhangfassaden / Fenster / Sonstige Fenster", "name": "OEKOBAU.DAT"}}, {"dataSetInternalID": 2, "referenceToFlowDataSet": {"shortDescription": [{"value": "Komponenten für die Wiederverwendung (CRU)", "lang": "de"}, {"value": "Components for re-use (CRU)", "lang": "en"}, {"value": "Componentes para su reutilización (CRU)", "lang": "es"}, {"value": "Komponenter för återanvändning (CRU)", "lang": "sv"}], "type": "flow data set", "refObjectId": "a2b32f97-3fc7-4af2-b209-525bc6426f33", "version": "30.00.002"}, "exchange direction": "OUTPUT", "meanAmount": 0.0, "other": {"anies": [{"value": "0.0", "module": "A1", "scenario": "Standard scenario"}, {"value": "0.0", "module": "A2", "scenario": "Standard scenario"}, {"value": "0.0", "module": "A3", "scenario": "Standard scenario"}, {"value": "0.0", "module": "A1-A3", "scenario": "Standard scenario"}, {"value": "0.0", "module": "A4", "scenario": "Standard scenario"}, {"value": "0.0", "module": "A5", "scenario": "Standard scenario"}, {"value": "0.0", "module": "C1", "scenario": "Standard scenario"}, {"value": "0.0", "module": "C2", "scenario": "Standard scenario"}, {"value": "0.0", "module": "C3", "scenario": "Standard scenario"}, {"value": "0.0", "module": "C4", "scenario": "Standard scenario"}, {"value": "0.0", "module": "D", "scenario": "Standard scenario"}, {"name": "referenceToUnitGroupDataSet", "value": {"shortDescription": [{"value": "kg"}], "type": "unit group data set", "refObjectId": "ad38d542-3fe9-439d-9b95-2f5f7752acaf", "uri": "../unitgroups/ad38d542-3fe9-439d-9b95-2f5f7752acaf"}}]}, "resolvedFlowVersion": "38.00.000", "flowProperties": [], "typeOfFlow": "Other flow", "classification": {"classHierarchy": "Quantities / Environmental quantities / EPD EN 15804 / LCI indicators", "name": "GaBiCategories"}}, {"dataSetInternalID": 3, "referenceToFlowDataSet": {"shortDescription": [{"value": "Exportierte elektrische Energie (EEE)", "lang": "de"}, {"value": "Exported electrical energy (EEE)", "lang": "en"}, {"value": "Energía exportada electrica (EEE)", "lang": "es"}, {"value": "Exporterad energi – elektrisk (EEE)", "lang": "sv"}], "type": "flow data set", "refObjectId": "4da0c987-2b76-40d6-9e9e-82a017aaaf29", "version": "30.00.002"}, "exchange direction": "OUTPUT", "meanAmount": 0.0, "other": {"anies": [{"value": "0.0", "module": "A1", "scenario": "Standard scenario"}, {"value": "0.0", "module": "A2", "scenario": "Standard scenario"}, {"value": "0.0", "module": "A3", "scenario": "Standard scenario"}, {"value": "0.0", "module": "A1-A3", "scenario": "Standard scenario"}, {"value": "0.0", "module": "A4", "scenario": "Standard scenario"}, {"value": "0.0", "module": "A5", "scenario": "Standard scenario"}, {"value": "0.0", "module": "C1", "scenario": "Standard scenario"}, {"value": "0.0", "module": "C2", "scenario": "Standard scenario"}, {"value": "0.0", "module": "C3", "scenario": "Standard scenario"}, {"value": "0.0", "module": "C4", "scenario": "Standard scenario"}, {"value": "-68.18870178", "module": "D", "scenario": "Standard scenario"}, {"name": "referenceToUnitGroupDataSet", "value": {"shortDescription": [{"value": "MJ"}], "type": "unit group data set", "refObjectId": "93a60a57-a3c8-11da-a746-0800200c9a66", "uri": "../unitgroups/93a60a57-a3c8-11da-a746-0800200c9a66"}}]}, "resolvedFlowVersion": "38.00.000", "flowProperties": [], "typeOfFlow": "Other flow", "classification": {"classHierarchy": "Quantities / Environmental quantities / EPD EN 15804 / LCI indicators", "name": "GaBiCategories"}}, {"dataSetInternalID": 4, "referenceToFlowDataSet": {"shortDescription": [{"value": "Exportierte thermische Energie (EET)", "lang": "de"}, {"value": "Exported thermal energy (EET)", "lang": "en"}, {"value": "Energía exportada termal (EET)", "lang": "es"}, {"value": "Exporterad energi – termisk (EET)", "lang": "sv"}], "type": "flow data set", "refObjectId": "98daf38a-7a79-46d3-9a37-2b7bd0955810", "version": "30.00.002"}, "exchange direction": "OUTPUT", "meanAmount": 0.0, "other": {"anies": [{"value": "0.0", "module": "A1", "scenario": "Standard scenario"}, {"value": "0.0", "module": "A2", "scenario": "Standard scenario"}, {"value": "0.0", "module": "A3", "scenario": "Standard scenario"}, {"value": "0.0", "module": "A1-A3", "scenario": "Standard scenario"}, {"value": "0.0", "module": "A4", "scenario": "Standard scenario"}, {"value": "0.0", "module": "A5", "scenario": "Standard scenario"}, {"value": "0.0", "module": "C1", "scenario": "Standard scenario"}, {"value": "0.0", "module": "C2", "scenario": "Standard scenario"}, {"value": "0.0", "module": "C3", "scenario": "Standard scenario"}, {"value": "0.0", "module": "C4", "scenario": "Standard scenario"}, {"value": "-117.4360975", "module": "D", "scenario": "Standard scenario"}, {"name": "referenceToUnitGroupDataSet", "value": {"shortDescription": [{"value": "MJ"}], "type": "unit group data set", "refObjectId": "93a60a57-a3c8-11da-a746-0800200c9a66", "uri": "../unitgroups/93a60a57-a3c8-11da-a746-0800200c9a66"}}]}, "resolvedFlowVersion": "38.00.000", "flowProperties": [], "typeOfFlow": "Other flow", "classification": {"classHierarchy": "Quantities / Environmental quantities / EPD EN 15804 / LCI indicators", "name": "GaBiCategories"}}, {"dataSetInternalID": 5, "referenceToFlowDataSet": {"shortDescription": [{"value": "Gefährlicher Abfall zur Deponie (HWD)", "lang": "de"}, {"value": "Hazardous waste disposed (HWD)", "lang": "en"}, {"value": "Residuos peligrosos eliminados (HWD)", "lang": "es"}, {"value": "Farligt avfall (HWD)", "lang": "sv"}], "type": "flow data set", "refObjectId": "430f9e0f-59b2-46a0-8e0d-55e0e84948fc", "version": "30.00.002"}, "exchange direction": "OUTPUT", "meanAmount": 0.0, "other": {"anies": [{"value": "0.152546789318812", "module": "A1", "scenario": "Standard scenario"}, {"value": "1.72464E-4", "module": "A2", "scenario": "Standard scenario"}, {"value": "0.050247863", "module": "A3", "scenario": "Standard scenario"}, {"value": "0.202967116318812", "module": "A1-A3", "scenario": "Standard scenario"}, {"value": "2.22748E-4", "module": "A4", "scenario": "Standard scenario"}, {"value": "3.66089E-5", "module": "A5", "scenario": "Standard scenario"}, {"value": "8.8284E-6", "module": "C1", "scenario": "Standard scenario"}, {"value": "2.96612E-5", "module": "C2", "scenario": "Standard scenario"}, {"value": "0.177129421909862", "module": "C3", "scenario": "Standard scenario"}, {"value": "3.40261E-6", "module": "C4", "scenario": "Standard scenario"}, {"value": "0.21760986031217", "module": "D", "scenario": "Standard scenario"}, {"name": "referenceToUnitGroupDataSet", "value": {"shortDescription": [{"value": "kg"}], "type": "unit group data set", "refObjectId": "ad38d542-3fe9-439d-9b95-2f5f7752acaf", "uri": "../unitgroups/ad38d542-3fe9-439d-9b95-2f5f7752acaf"}}]}, "resolvedFlowVersion": "38.00.000", "flowProperties": [], "typeOfFlow": "Other flow", "classification": {"classHierarchy": "Quantities / Environmental quantities / EPD EN 15804 / LCI indicators", "name": "GaBiCategories"}}, {"dataSetInternalID": 6, "referenceToFlowDataSet": {"shortDescription": [{"value": "Stoffe für die Energierückgewinnung (MER)", "lang": "de"}, {"value": "Materials for energy recovery (MER)", "lang": "en"}, {"value": "Materiales para valorización energética (recuperación de energía) (MER)", "lang": "es"}, {"value": "Material till energiåtervinning (MER)", "lang": "sv"}], "type": "flow data set", "refObjectId": "59a9181c-3aaf-46ee-8b13-2b3723b6e447", "version": "30.00.002"}, "exchange direction": "OUTPUT", "meanAmount": 0.0, "other": {"anies": [{"value": "0.0", "module": "A1", "scenario": "Standard scenario"}, {"value": "0.0", "module": "A2", "scenario": "Standard scenario"}, {"value": "0.0", "module": "A3", "scenario": "Standard scenario"}, {"value": "0.0", "module": "A1-A3", "scenario": "Standard scenario"}, {"value": "0.0", "module": "A4", "scenario": "Standard scenario"}, {"value": "0.0", "module": "A5", "scenario": "Standard scenario"}, {"value": "0.0", "module": "C1", "scenario": "Standard scenario"}, {"value": "0.0", "module": "C2", "scenario": "Standard scenario"}, {"value": "0.0", "module": "C3", "scenario": "Standard scenario"}, {"value": "0.0", "module": "C4", "scenario": "Standard scenario"}, {"value": "0.0", "module": "D", "scenario": "Standard scenario"}, {"name": "referenceToUnitGroupDataSet", "value": {"shortDescription": [{"value": "kg"}], "type": "unit group data set", "refObjectId": "ad38d542-3fe9-439d-9b95-2f5f7752acaf", "uri": "../unitgroups/ad38d542-3fe9-439d-9b95-2f5f7752acaf"}}]}, "resolvedFlowVersion": "38.00.000", "flowProperties": [], "typeOfFlow": "Other flow", "classification": {"classHierarchy": "Quantities / Environmental quantities / EPD EN 15804 / LCI indicators", "name": "GaBiCategories"}}, {"dataSetInternalID": 7, "referenceToFlowDataSet": {"shortDescription": [{"value": "Stoffe zum Recycling (MFR)", "lang": "de"}, {"value": "Materials for recycling (MFR)", "lang": "en"}, {"value": "Materiales para el reciclaje (MFR)", "lang": "es"}, {"value": "Material till återvinning (MFR)", "lang": "sv"}], "type": "flow data set", "refObjectId": "d7fe48a5-4103-49c8-9aae-b0b5dfdbd6ae", "version": "30.00.002"}, "exchange direction": "OUTPUT", "meanAmount": 0.0, "other": {"anies": [{"value": "0.0", "module": "A1", "scenario": "Standard scenario"}, {"value": "0.0", "module": "A2", "scenario": "Standard scenario"}, {"value": "2.448212", "module": "A3", "scenario": "Standard scenario"}, {"value": "2.448212", "module": "A1-A3", "scenario": "Standard scenario"}, {"value": "0.0", "module": "A4", "scenario": "Standard scenario"}, {"value": "1.25", "module": "A5", "scenario": "Standard scenario"}, {"value": "0.0", "module": "C1", "scenario": "Standard scenario"}, {"value": "0.0", "module": "C2", "scenario": "Standard scenario"}, {"value": "62.78165", "module": "C3", "scenario": "Standard scenario"}, {"value": "0.0", "module": "C4", "scenario": "Standard scenario"}, {"value": "0.0", "module": "D", "scenario": "Standard scenario"}, {"name": "referenceToUnitGroupDataSet", "value": {"shortDescription": [{"value": "kg"}], "type": "unit group data set", "refObjectId": "ad38d542-3fe9-439d-9b95-2f5f7752acaf", "uri": "../unitgroups/ad38d542-3fe9-439d-9b95-2f5f7752acaf"}}]}, "resolvedFlowVersion": "38.00.000", "flowProperties": [], "typeOfFlow": "Other flow", "classification": {"classHierarchy": "Quantities / Environmental quantities / EPD EN 15804 / LCI indicators", "name": "GaBiCategories"}}, {"dataSetInternalID": 8, "referenceToFlowDataSet": {"shortDescription": [{"value": "Einsatz von Süßwasserressourcen (FW)", "lang": "de"}, {"value": "Use of net fresh water (FW)", "lang": "en"}, {"value": "Uso neto de recursos de agua dulce (FW)", "lang": "es"}, {"value": "Användning av sötvatten (FW)", "lang": "sv"}], "type": "flow data set", "refObjectId": "3cf952c8-f3a4-461d-8c96-96456ca62246", "version": "30.00.003"}, "exchange direction": "INPUT", "meanAmount": 0.0, "other": {"anies": [{"value": "5.63810090126419", "module": "A1", "scenario": "Standard scenario"}, {"value": "0.008290219", "module": "A2", "scenario": "Standard scenario"}, {"value": "0.405630778336098", "module": "A3", "scenario": "Standard scenario"}, {"value": "6.052021898600288", "module": "A1-A3", "scenario": "Standard scenario"}, {"value": "0.010807347", "module": "A4", "scenario": "Standard scenario"}, {"value": "0.026350739", "module": "A5", "scenario": "Standard scenario"}, {"value": "0.011082569", "module": "C1", "scenario": "Standard scenario"}, {"value": "0.001425792", "module": "C2", "scenario": "Standard scenario"}, {"value": "0.048307319", "module": "C3", "scenario": "Standard scenario"}, {"value": "0.003211337", "module": "C4", "scenario": "Standard scenario"}, {"value": "-1.949423023", "module": "D", "scenario": "Standard scenario"}, {"name": "referenceToUnitGroupDataSet", "value": {"shortDescription": [{"value": "m3"}], "type": "unit group data set", "refObjectId": "cd950537-0a98-4044-9ba7-9f9a68d0a504", "uri": "../unitgroups/cd950537-0a98-4044-9ba7-9f9a68d0a504"}}]}, "resolvedFlowVersion": "38.00.000", "flowProperties": [], "typeOfFlow": "Other flow", "classification": {"classHierarchy": "Quantities / Environmental quantities / EPD EN 15804 / LCI indicators", "name": "GaBiCategories"}}, {"dataSetInternalID": 9, "referenceToFlowDataSet": {"shortDescription": [{"value": "Entsorgter nicht gefährlicher Abfall (NHWD)", "lang": "de"}, {"value": "Non hazardous waste dispose (NHWD)", "lang": "en"}, {"value": "Residuos no peligrosos eliminados (NHWD)", "lang": "es"}, {"value": "Icke-farligt avfall (NHWD)", "lang": "sv"}], "type": "flow data set", "refObjectId": "b29ef66b-e286-4afa-949f-62f1a7b4d7fa", "version": "30.00.002"}, "exchange direction": "OUTPUT", "meanAmount": 0.0, "other": {"anies": [{"value": "143.01098818532", "module": "A1", "scenario": "Standard scenario"}, {"value": "4.31711993965895", "module": "A2", "scenario": "Standard scenario"}, {"value": "8.11005571720153", "module": "A3", "scenario": "Standard scenario"}, {"value": "155.43816384218047", "module": "A1-A3", "scenario": "Standard scenario"}, {"value": "5.88628840926449", "module": "A4", "scenario": "Standard scenario"}, {"value": "3.3924625903902", "module": "A5", "scenario": "Standard scenario"}, {"value": "0.044820059", "module": "C1", "scenario": "Standard scenario"}, {"value": "0.742478986512848", "module": "C2", "scenario": "Standard scenario"}, {"value": "3.38500807215849", "module": "C3", "scenario": "Standard scenario"}, {"value": "18.0105635809999", "module": "C4", "scenario": "Standard scenario"}, {"value": "-68.27144461", "module": "D", "scenario": "Standard scenario"}, {"name": "referenceToUnitGroupDataSet", "value": {"shortDescription": [{"value": "kg"}], "type": "unit group data set", "refObjectId": "ad38d542-3fe9-439d-9b95-2f5f7752acaf", "uri": "../unitgroups/ad38d542-3fe9-439d-9b95-2f5f7752acaf"}}]}, "resolvedFlowVersion": "38.00.000", "flowProperties": [], "typeOfFlow": "Other flow", "classification": {"classHierarchy": "Quantities / Environmental quantities / EPD EN 15804 / LCI indicators", "name": "GaBiCategories"}}, {"dataSetInternalID": 10, "referenceToFlowDataSet": {"shortDescription": [{"value": "Nicht-erneuerbare Primärenergie als Energieträger (PENRE)", "lang": "de"}, {"value": "Use of non renewable primary energy (PENRE)", "lang": "en"}, {"value": "Uso de energía primaria no renovable, excluyendo los recursos de energía primaria no renovable utilizada como materia prima (PENRE)", "lang": "es"}, {"value": "Icke förnybar primärenergi - använd som energibärare (PENRE)", "lang": "sv"}], "type": "flow data set", "refObjectId": "ac857178-2b45-46ec-892a-a9a4332f0372", "version": "30.00.002"}, "exchange direction": "INPUT", "meanAmount": 0.0, "other": {"anies": [{"value": "8373.93", "module": "A1", "scenario": "Standard scenario"}, {"value": "72.2587125391305", "module": "A2", "scenario": "Standard scenario"}, {"value": "561.373070620073", "module": "A3", "scenario": "Standard scenario"}, {"value": "9007.561783159204", "module": "A1-A3", "scenario": "Standard scenario"}, {"value": "92.8890556713379", "module": "A4", "scenario": "Standard scenario"}, {"value": "26.3745165047716", "module": "A5", "scenario": "Standard scenario"}, {"value": "13.901697991147", "module": "C1", "scenario": "Standard scenario"}, {"value": "12.4273998412504", "module": "C2", "scenario": "Standard scenario"}, {"value": "71.9168363838499", "module": "C3", "scenario": "Standard scenario"}, {"value": "3.02460773975", "module": "C4", "scenario": "Standard scenario"}, {"value": "-3653.04", "module": "D", "scenario": "Standard scenario"}, {"name": "referenceToUnitGroupDataSet", "value": {"shortDescription": [{"value": "MJ"}], "type": "unit group data set", "refObjectId": "93a60a57-a3c8-11da-a746-0800200c9a66", "uri": "../unitgroups/93a60a57-a3c8-11da-a746-0800200c9a66"}}]}, "resolvedFlowVersion": "38.00.000", "flowProperties": [], "typeOfFlow": "Other flow", "classification": {"classHierarchy": "Quantities", "name": "GaBiCategories"}}, {"dataSetInternalID": 11, "referenceToFlowDataSet": {"shortDescription": [{"value": "Nicht-erneuerbare Primärenergie zur stofflichen Nutzung (PENRM)", "lang": "de"}, {"value": "Use of non renewable primary energy resources used as raw materials (PENRM)", "lang": "en"}, {"value": "Uso de la energía primaria no renovable utilizada como materia prima (PENRM)", "lang": "es"}, {"value": "Icke förnybar primärenergi - använd som råmaterial (PENRM)", "lang": "sv"}], "type": "flow data set", "refObjectId": "1421caa0-679d-4bf4-b282-0eb850ccae27", "version": "30.00.001"}, "exchange direction": "INPUT", "meanAmount": 0.0, "other": {"anies": [{"value": "80.039", "module": "A1", "scenario": "Standard scenario"}, {"value": "0.0", "module": "A2", "scenario": "Standard scenario"}, {"value": "22.9499999999999", "module": "A3", "scenario": "Standard scenario"}, {"value": "102.9889999999999", "module": "A1-A3", "scenario": "Standard scenario"}, {"value": "0.0", "module": "A4", "scenario": "Standard scenario"}, {"value": "0.0", "module": "A5", "scenario": "Standard scenario"}, {"value": "0.0", "module": "C1", "scenario": "Standard scenario"}, {"value": "0.0", "module": "C2", "scenario": "Standard scenario"}, {"value": "0.0", "module": "C3", "scenario": "Standard scenario"}, {"value": "0.0", "module": "C4", "scenario": "Standard scenario"}, {"value": "-1.06705875", "module": "D", "scenario": "Standard scenario"}, {"name": "referenceToUnitGroupDataSet", "value": {"shortDescription": [{"value": "MJ"}], "type": "unit group data set", "refObjectId": "93a60a57-a3c8-11da-a746-0800200c9a66", "uri": "../unitgroups/93a60a57-a3c8-11da-a746-0800200c9a66"}}]}, "resolvedFlowVersion": "38.00.000", "flowProperties": [], "typeOfFlow": "Other flow", "classification": {"classHierarchy": "Quantities", "name": "GaBiCategories"}}, {"dataSetInternalID": 12, "referenceToFlowDataSet": {"shortDescription": [{"value": "Nicht erneuerbare Sekundärbrennstoffe (NRSF)", "lang": "de"}, {"value": "Use of non renewable secondary fuels (NRSF)", "lang": "en"}, {"value": "Uso de combustibles secundarios no renovables (NRSF)", "lang": "es"}, {"value": "Användning av ickeförnybara sekundära bränslen (NRSF)", "lang": "sv"}], "type": "flow data set", "refObjectId": "89def144-d39a-4287-b86f-efde453ddcb2", "version": "30.00.001"}, "exchange direction": "INPUT", "meanAmount": 0.0, "other": {"anies": [{"value": "0.0", "module": "A1", "scenario": "Standard scenario"}, {"value": "0.0", "module": "A2", "scenario": "Standard scenario"}, {"value": "0.0", "module": "A3", "scenario": "Standard scenario"}, {"value": "0.0", "module": "A1-A3", "scenario": "Standard scenario"}, {"value": "0.0", "module": "A4", "scenario": "Standard scenario"}, {"value": "0.0", "module": "A5", "scenario": "Standard scenario"}, {"value": "0.0", "module": "C1", "scenario": "Standard scenario"}, {"value": "0.0", "module": "C2", "scenario": "Standard scenario"}, {"value": "0.0", "module": "C3", "scenario": "Standard scenario"}, {"value": "0.0", "module": "C4", "scenario": "Standard scenario"}, {"value": "0.0", "module": "D", "scenario": "Standard scenario"}, {"name": "referenceToUnitGroupDataSet", "value": {"shortDescription": [{"value": "MJ"}], "type": "unit group data set", "refObjectId": "93a60a57-a3c8-11da-a746-0800200c9a66", "uri": "../unitgroups/93a60a57-a3c8-11da-a746-0800200c9a66"}}]}, "resolvedFlowVersion": "38.00.000", "flowProperties": [], "typeOfFlow": "Other flow", "classification": {"classHierarchy": "Quantities / Environmental quantities / EPD EN 15804 / LCI indicators", "name": "GaBiCategories"}}, {"dataSetInternalID": 13, "referenceToFlowDataSet": {"shortDescription": [{"value": "Entsorgter radioaktiver Abfall (RWD)", "lang": "de"}, {"value": "Radioactive waste disposed (RWD)", "lang": "en"}, {"value": "Residuos radiactivos eliminados (RWD)", "lang": "es"}, {"value": "Radioaktivt avfall (RWD) ", "lang": "sv"}], "type": "flow data set", "refObjectId": "3449546e-52ad-4b39-b809-9fb77cea8ff6", "version": "30.00.001"}, "exchange direction": "OUTPUT", "meanAmount": 0.0, "other": {"anies": [{"value": "0.023494127", "module": "A1", "scenario": "Standard scenario"}, {"value": "4.46908E-4", "module": "A2", "scenario": "Standard scenario"}, {"value": "0.001472716", "module": "A3", "scenario": "Standard scenario"}, {"value": "0.025413751", "module": "A1-A3", "scenario": "Standard scenario"}, {"value": "5.91541E-4", "module": "A4", "scenario": "Standard scenario"}, {"value": "1.59447E-4", "module": "A5", "scenario": "Standard scenario"}, {"value": "9.40187E-5", "module": "C1", "scenario": "Standard scenario"}, {"value": "7.68615E-5", "module": "C2", "scenario": "Standard scenario"}, {"value": "3.24379E-4", "module": "C3", "scenario": "Standard scenario"}, {"value": "1.83647E-5", "module": "C4", "scenario": "Standard scenario"}, {"value": "-0.005314263", "module": "D", "scenario": "Standard scenario"}, {"name": "referenceToUnitGroupDataSet", "value": {"shortDescription": [{"value": "kg"}], "type": "unit group data set", "refObjectId": "ad38d542-3fe9-439d-9b95-2f5f7752acaf", "uri": "../unitgroups/ad38d542-3fe9-439d-9b95-2f5f7752acaf"}}]}, "resolvedFlowVersion": "38.00.000", "flowProperties": [], "typeOfFlow": "Other flow", "classification": {"classHierarchy": "Quantities / Environmental quantities / EPD EN 15804 / LCI indicators", "name": "GaBiCategories"}}, {"dataSetInternalID": 14, "referenceToFlowDataSet": {"shortDescription": [{"value": "Erneuerbare Primärenergie als Energieträger (PERE)", "lang": "de"}, {"value": "Use of renewable primary energy (PERE)", "lang": "en"}, {"value": "Uso de energía primaria renovable excluyendo los recursos de energía primaria renovable utilizada como materia prima (PERE)", "lang": "es"}, {"value": "Förnybar energi - använd som energibärare (PERE)", "lang": "sv"}], "type": "flow data set", "refObjectId": "20f32be5-0398-4288-9b6d-accddd195317", "version": "30.00.001"}, "exchange direction": "INPUT", "meanAmount": 0.0, "other": {"anies": [{"value": "970.36138029633", "module": "A1", "scenario": "Standard scenario"}, {"value": "0.852036320883505", "module": "A2", "scenario": "Standard scenario"}, {"value": "442.706599931381", "module": "A3", "scenario": "Standard scenario"}, {"value": "1413.9200165485945", "module": "A1-A3", "scenario": "Standard scenario"}, {"value": "1.36962537495661", "module": "A4", "scenario": "Standard scenario"}, {"value": "2.90620173308612", "module": "A5", "scenario": "Standard scenario"}, {"value": "2.5101070543751", "module": "C1", "scenario": "Standard scenario"}, {"value": "0.14653729172317", "module": "C2", "scenario": "Standard scenario"}, {"value": "7.20894640889999", "module": "C3", "scenario": "Standard scenario"}, {"value": "0.058878013", "module": "C4", "scenario": "Standard scenario"}, {"value": "-765.257532", "module": "D", "scenario": "Standard scenario"}, {"name": "referenceToUnitGroupDataSet", "value": {"shortDescription": [{"value": "MJ"}], "type": "unit group data set", "refObjectId": "93a60a57-a3c8-11da-a746-0800200c9a66", "uri": "../unitgroups/93a60a57-a3c8-11da-a746-0800200c9a66"}}]}, "resolvedFlowVersion": "38.00.000", "flowProperties": [], "typeOfFlow": "Other flow", "classification": {"classHierarchy": "Quantities", "name": "GaBiCategories"}}, {"dataSetInternalID": 15, "referenceToFlowDataSet": {"shortDescription": [{"value": "Erneuerbare Primärenergie zur stofflichen Nutzung (PERM)", "lang": "de"}, {"value": "Use of renewable primary energy resources used as raw materials (PERM)", "lang": "en"}, {"value": "Uso de energía primaria renovable utilizada como materia prima (PERM)", "lang": "es"}, {"value": "Förnybar energi - använd som råmaterial (PERM)", "lang": "sv"}], "type": "flow data set", "refObjectId": "fb3ec0de-548d-4508-aea5-00b73bf6f702", "version": "30.00.001"}, "exchange direction": "INPUT", "meanAmount": 0.0, "other": {"anies": [{"value": "0.0", "module": "A1", "scenario": "Standard scenario"}, {"value": "0.0", "module": "A2", "scenario": "Standard scenario"}, {"value": "349.75", "module": "A3", "scenario": "Standard scenario"}, {"value": "349.75", "module": "A1-A3", "scenario": "Standard scenario"}, {"value": "0.0", "module": "A4", "scenario": "Standard scenario"}, {"value": "0.0", "module": "A5", "scenario": "Standard scenario"}, {"value": "0.0", "module": "C1", "scenario": "Standard scenario"}, {"value": "0.0", "module": "C2", "scenario": "Standard scenario"}, {"value": "0.0", "module": "C3", "scenario": "Standard scenario"}, {"value": "0.0", "module": "C4", "scenario": "Standard scenario"}, {"value": "0.0", "module": "D", "scenario": "Standard scenario"}, {"name": "referenceToUnitGroupDataSet", "value": {"shortDescription": [{"value": "MJ"}], "type": "unit group data set", "refObjectId": "93a60a57-a3c8-11da-a746-0800200c9a66", "uri": "../unitgroups/93a60a57-a3c8-11da-a746-0800200c9a66"}}]}, "resolvedFlowVersion": "38.00.000", "flowProperties": [], "typeOfFlow": "Other flow", "classification": {"classHierarchy": "Quantities", "name": "GaBiCategories"}}, {"dataSetInternalID": 16, "referenceToFlowDataSet": {"shortDescription": [{"value": "Erneuerbare Sekundärbrennstoffe (RSF)", "lang": "de"}, {"value": "Use of renewable secondary fuels (RSF)", "lang": "en"}, {"value": "Uso de combustibles secundarios renovables (RSF)", "lang": "es"}, {"value": "Användning av förnybara sekundära bränslen (RSF)", "lang": "sv"}], "type": "flow data set", "refObjectId": "64333088-a55f-4aa2-9a31-c10b07816787", "version": "30.00.001"}, "exchange direction": "INPUT", "meanAmount": 0.0, "other": {"anies": [{"value": "0.0", "module": "A1", "scenario": "Standard scenario"}, {"value": "0.0", "module": "A2", "scenario": "Standard scenario"}, {"value": "0.0", "module": "A3", "scenario": "Standard scenario"}, {"value": "0.0", "module": "A1-A3", "scenario": "Standard scenario"}, {"value": "0.0", "module": "A4", "scenario": "Standard scenario"}, {"value": "0.0", "module": "A5", "scenario": "Standard scenario"}, {"value": "0.0", "module": "C1", "scenario": "Standard scenario"}, {"value": "0.0", "module": "C2", "scenario": "Standard scenario"}, {"value": "0.0", "module": "C3", "scenario": "Standard scenario"}, {"value": "0.0", "module": "C4", "scenario": "Standard scenario"}, {"value": "0.0", "module": "D", "scenario": "Standard scenario"}, {"name": "referenceToUnitGroupDataSet", "value": {"shortDescription": [{"value": "MJ"}], "type": "unit group data set", "refObjectId": "93a60a57-a3c8-11da-a746-0800200c9a66", "uri": "../unitgroups/93a60a57-a3c8-11da-a746-0800200c9a66"}}]}, "resolvedFlowVersion": "38.00.000", "flowProperties": [], "typeOfFlow": "Other flow", "classification": {"classHierarchy": "Quantities / Environmental quantities / EPD EN 15804 / LCI indicators", "name": "GaBiCategories"}}, {"dataSetInternalID": 17, "referenceToFlowDataSet": {"shortDescription": [{"value": "Einsatz von Sekundärstoffen (SM)", "lang": "de"}, {"value": "Use of secondary material (SM)", "lang": "en"}, {"value": "Uso de materiales secundarios (SM)", "lang": "es"}, {"value": "Användning av sekundära material (SM)", "lang": "sv"}], "type": "flow data set", "refObjectId": "c6a1f35f-2d09-4f54-8dfb-97e502e1ce92", "version": "30.00.001"}, "exchange direction": "INPUT", "meanAmount": 0.0, "other": {"anies": [{"value": "3.13", "module": "A1", "scenario": "Standard scenario"}, {"value": "0.0", "module": "A2", "scenario": "Standard scenario"}, {"value": "0.00106", "module": "A3", "scenario": "Standard scenario"}, {"value": "3.13", "module": "A1-A3", "scenario": "Standard scenario"}, {"value": "0.0", "module": "A4", "scenario": "Standard scenario"}, {"value": "0.0", "module": "A5", "scenario": "Standard scenario"}, {"value": "0.0", "module": "C1", "scenario": "Standard scenario"}, {"value": "0.0", "module": "C2", "scenario": "Standard scenario"}, {"value": "0.0", "module": "C3", "scenario": "Standard scenario"}, {"value": "0.0", "module": "C4", "scenario": "Standard scenario"}, {"value": "0.0134", "module": "D", "scenario": "Standard scenario"}, {"name": "referenceToUnitGroupDataSet", "value": {"shortDescription": [{"value": "kg"}], "type": "unit group data set", "refObjectId": "ad38d542-3fe9-439d-9b95-2f5f7752acaf", "uri": "../unitgroups/ad38d542-3fe9-439d-9b95-2f5f7752acaf"}}]}, "resolvedFlowVersion": "38.00.000", "flowProperties": [], "typeOfFlow": "Other flow", "classification": {"classHierarchy": "Quantities / Environmental quantities / EPD EN 15804 / LCI indicators", "name": "GaBiCategories"}}, {"dataSetInternalID": 18, "referenceToFlowDataSet": {"shortDescription": [{"value": "Total nicht erneuerbare Primärenergie (PENRT)", "lang": "de"}, {"value": "Total use of non renewable primary energy resource (PENRT)", "lang": "en"}, {"value": "Uso total de la energía primaria no renovable (energía primaria y recursos de energía primaria renovable utilizada como materia prima) (PENRT)", "lang": "es"}, {"value": "Icke förnybar primärenergi – total (PENRT)", "lang": "sv"}], "type": "flow data set", "refObjectId": "06159210-646b-4c8d-8583-da9b3b95a6c1", "version": "30.00.001"}, "exchange direction": "INPUT", "meanAmount": 0.0, "other": {"anies": [{"value": "8454.33", "module": "A1", "scenario": "Standard scenario"}, {"value": "72.2587125391305", "module": "A2", "scenario": "Standard scenario"}, {"value": "584.323070620073", "module": "A3", "scenario": "Standard scenario"}, {"value": "9110.911783159205", "module": "A1-A3", "scenario": "Standard scenario"}, {"value": "92.8890556713379", "module": "A4", "scenario": "Standard scenario"}, {"value": "26.3745165047716", "module": "A5", "scenario": "Standard scenario"}, {"value": "13.901697991147", "module": "C1", "scenario": "Standard scenario"}, {"value": "12.4273998412504", "module": "C2", "scenario": "Standard scenario"}, {"value": "73.772696767325", "module": "C3", "scenario": "Standard scenario"}, {"value": "3.066457797125", "module": "C4", "scenario": "Standard scenario"}, {"value": "-3653.7", "module": "D", "scenario": "Standard scenario"}, {"name": "referenceToUnitGroupDataSet", "value": {"shortDescription": [{"value": "MJ"}], "type": "unit group data set", "refObjectId": "93a60a57-a3c8-11da-a746-0800200c9a66", "uri": "../unitgroups/93a60a57-a3c8-11da-a746-0800200c9a66"}}]}, "resolvedFlowVersion": "38.00.000", "flowProperties": [], "typeOfFlow": "Other flow", "classification": {"classHierarchy": "Quantities / Environmental quantities / EPD EN 15804 / LCI indicators", "name": "GaBiCategories"}}, {"dataSetInternalID": 19, "referenceToFlowDataSet": {"shortDescription": [{"value": "Total erneuerbare Primärenergie (PERT)", "lang": "de"}, {"value": "Total use of renewable primary energy resources (PERT)", "lang": "en"}, {"value": "Uso total de la energía primaria renovable (energía primaria y recursos de energía primaria renovable utilizada como materia prima) (PERT)", "lang": "es"}, {"value": "Förnybar energi – total (PERT)", "lang": "sv"}], "type": "flow data set", "refObjectId": "53f97275-fa8a-4cdd-9024-65936002acd0", "version": "30.00.001"}, "exchange direction": "INPUT", "meanAmount": 0.0, "other": {"anies": [{"value": "970.36138029633", "module": "A1", "scenario": "Standard scenario"}, {"value": "0.852036320883505", "module": "A2", "scenario": "Standard scenario"}, {"value": "792.456599931381", "module": "A3", "scenario": "Standard scenario"}, {"value": "1763.6700165485945", "module": "A1-A3", "scenario": "Standard scenario"}, {"value": "1.36962537495661", "module": "A4", "scenario": "Standard scenario"}, {"value": "2.90620173308612", "module": "A5", "scenario": "Standard scenario"}, {"value": "2.5101070543751", "module": "C1", "scenario": "Standard scenario"}, {"value": "0.14653729172317", "module": "C2", "scenario": "Standard scenario"}, {"value": "7.37319498293324", "module": "C3", "scenario": "Standard scenario"}, {"value": "0.059611797", "module": "C4", "scenario": "Standard scenario"}, {"value": "-765.1340016", "module": "D", "scenario": "Standard scenario"}, {"name": "referenceToUnitGroupDataSet", "value": {"shortDescription": [{"value": "MJ"}], "type": "unit group data set", "refObjectId": "93a60a57-a3c8-11da-a746-0800200c9a66", "uri": "../unitgroups/93a60a57-a3c8-11da-a746-0800200c9a66"}}]}, "resolvedFlowVersion": "38.00.000", "flowProperties": [], "typeOfFlow": "Other flow", "classification": {"classHierarchy": "Quantities / Environmental quantities / EPD EN 15804 / LCI indicators", "name": "GaBiCategories"}}]}, "LCIAResults": {"LCIAResult": [{"referenceToLCIAMethodDataSet": {"shortDescription": [{"value": "Potenzial für die Verknappung abiotischer Ressourcen – nicht fossile Ressourcen (ADPE)", "lang": "de"}, {"value": "Abiotic depletion potential - non-fossil resources (ADPE)", "lang": "en"}, {"value": "Abiotisk utarmningspotential icke fossila resurser (ADP-mm)", "lang": "sv"}], "type": "LCIA method data set", "refObjectId": "b2ad6494-c78d-11e6-9d9d-cec0c932ce01", "version": "01.00.013"}, "meanAmount": 0.0, "other": {"anies": [{"value": "0.013557556", "module": "A1", "scenario": "Standard scenario"}, {"value": "1.14334E-4", "module": "A2", "scenario": "Standard scenario"}, {"value": "0.010879411", "module": "A3", "scenario": "Standard scenario"}, {"value": "0.024551301", "module": "A1-A3", "scenario": "Standard scenario"}, {"value": "1.63535E-4", "module": "A4", "scenario": "Standard scenario"}, {"value": "2.08632E-5", "module": "A5", "scenario": "Standard scenario"}, {"value": "4.68571E-6", "module": "C1", "scenario": "Standard scenario"}, {"value": "1.96637E-5", "module": "C2", "scenario": "Standard scenario"}, {"value": "1.62891E-4", "module": "C3", "scenario": "Standard scenario"}, {"value": "9.46002E-7", "module": "C4", "scenario": "Standard scenario"}, {"value": "0.106284798591289", "module": "D", "scenario": "Standard scenario"}, {"name": "referenceToUnitGroupDataSet", "value": {"shortDescription": [{"value": "kg Sb-Äqv."}], "type": "unit group data set", "refObjectId": "54ccd2d9-a32a-4fc2-923d-f2c8c93e89d4", "uri": "../unitgroups/54ccd2d9-a32a-4fc2-923d-f2c8c93e89d4"}}]}}, {"referenceToLCIAMethodDataSet": {"shortDescription": [{"value": "Potenzial für die Verknappung abiotischer Ressourcen – fossile Brennstoffe (ADPF)", "lang": "de"}, {"value": "Abiotic depletion potential - fossil resources (ADPF)", "lang": "en"}, {"value": "Abiotisk utarmningspotential av fossila resurser (ADP-F)", "lang": "sv"}], "type": "LCIA method data set", "refObjectId": "b2ad6110-c78d-11e6-9d9d-cec0c932ce01", "version": "01.00.012"}, "meanAmount": 0.0, "other": {"anies": [{"value": "7969.96", "module": "A1", "scenario": "Standard scenario"}, {"value": "68.0578853915436", "module": "A2", "scenario": "Standard scenario"}, {"value": "548.128939028247", "module": "A3", "scenario": "Standard scenario"}, {"value": "8586.146824419791", "module": "A1-A3", "scenario": "Standard scenario"}, {"value": "87.4961048865785", "module": "A4", "scenario": "Standard scenario"}, {"value": "24.9708424635099", "module": "A5", "scenario": "Standard scenario"}, {"value": "13.2503972378326", "module": "C1", "scenario": "Standard scenario"}, {"value": "11.704921446707", "module": "C2", "scenario": "Standard scenario"}, {"value": "69.0282888666499", "module": "C3", "scenario": "Standard scenario"}, {"value": "2.88703316779999", "module": "C4", "scenario": "Standard scenario"}, {"value": "-3440.94", "module": "D", "scenario": "Standard scenario"}, {"name": "referenceToUnitGroupDataSet", "value": {"shortDescription": [{"value": "MJ"}], "type": "unit group data set", "refObjectId": "93a60a57-a3c8-11da-a746-0800200c9a66", "uri": "../unitgroups/93a60a57-a3c8-11da-a746-0800200c9a66"}}]}}, {"referenceToLCIAMethodDataSet": {"shortDescription": [{"value": "Versauerungspotenzial, kumulierte Überschreitung (AP)", "lang": "de"}, {"value": "Acidification potential, Accumulated Exceedance (AP)", "lang": "en"}, {"value": "Försurningspotential på land och vatten (AP)", "lang": "sv"}], "type": "LCIA method data set", "refObjectId": "b5c611c6-def3-11e6-bf01-fe55135034f3", "version": "01.03.012", "uri": "http://lca.jrc.ec.europa.eu/lcainfohub/datasets/elcd/lciamethods/f6cbd466-253f-4145-a4bb-8dae7d266e89.xml"}, "meanAmount": 0.0, "other": {"anies": [{"value": "5.11027193568599", "module": "A1", "scenario": "Standard scenario"}, {"value": "0.026171466", "module": "A2", "scenario": "Standard scenario"}, {"value": "0.239538189784029", "module": "A3", "scenario": "Standard scenario"}, {"value": "5.375981591470019", "module": "A1-A3", "scenario": "Standard scenario"}, {"value": "0.017318092", "module": "A4", "scenario": "Standard scenario"}, {"value": "0.01446039", "module": "A5", "scenario": "Standard scenario"}, {"value": "0.003758079", "module": "C1", "scenario": "Standard scenario"}, {"value": "0.004501094", "module": "C2", "scenario": "Standard scenario"}, {"value": "0.039834864", "module": "C3", "scenario": "Standard scenario"}, {"value": "9.64706E-4", "module": "C4", "scenario": "Standard scenario"}, {"value": "-2.40525834", "module": "D", "scenario": "Standard scenario"}, {"name": "referenceToUnitGroupDataSet", "value": {"shortDescription": [{"value": "mol H+ eqv."}], "type": "unit group data set", "refObjectId": "42e089ac-92bf-4bf2-8ca1-5fc40d18f2ed", "uri": "../unitgroups/42e089ac-92bf-4bf2-8ca1-5fc40d18f2ed"}}]}}, {"referenceToLCIAMethodDataSet": {"shortDescription": [{"value": "Eutrophierungspotenzial - Süßwasser (EP-freshwater)", "lang": "de"}, {"value": "Eutrophication potential - freshwater (EP-freshwater)", "lang": "en"}, {"value": "Övergödningspotential sötvatten (EP-fw)", "lang": "sv"}], "type": "LCIA method data set", "refObjectId": "b53ec18f-7377-4ad3-86eb-cc3f4f276b2b", "version": "01.00.012", "uri": "http://lca.jrc.ec.europa.eu/lcainfohub/datasets/elcd/lciamethods/a4630d5b-df2f-48ae-b3f2-5e5257606d68.xml"}, "meanAmount": 0.0, "other": {"anies": [{"value": "0.026075842", "module": "A1", "scenario": "Standard scenario"}, {"value": "4.55207E-5", "module": "A2", "scenario": "Standard scenario"}, {"value": "0.001707222", "module": "A3", "scenario": "Standard scenario"}, {"value": "0.0278285847", "module": "A1-A3", "scenario": "Standard scenario"}, {"value": "5.09916E-5", "module": "A4", "scenario": "Standard scenario"}, {"value": "8.55858E-5", "module": "A5", "scenario": "Standard scenario"}, {"value": "6.87611E-5", "module": "C1", "scenario": "Standard scenario"}, {"value": "7.82887E-6", "module": "C2", "scenario": "Standard scenario"}, {"value": "2.58675E-4", "module": "C3", "scenario": "Standard scenario"}, {"value": "1.66782E-6", "module": "C4", "scenario": "Standard scenario"}, {"value": "-0.012061638", "module": "D", "scenario": "Standard scenario"}, {"name": "referenceToUnitGroupDataSet", "value": {"shortDescription": [{"value": "kg P eqv."}], "type": "unit group data set", "refObjectId": "0429039d-a61d-4590-ba67-aa4a20a810a1", "uri": "../unitgroups/0429039d-a61d-4590-ba67-aa4a20a810a1"}}]}}, {"referenceToLCIAMethodDataSet": {"shortDescription": [{"value": "Eutrophierungspotenzial - Salzwasser (EP-marine)", "lang": "de"}, {"value": "Eutrophication potential - marine (EP-marine)", "lang": "en"}, {"value": "Övergödningspotential marin (EP-m)", "lang": "sv"}], "type": "LCIA method data set", "refObjectId": "b5c619fa-def3-11e6-bf01-fe55135034f3", "version": "02.00.012", "uri": "http://lca.jrc.ec.europa.eu/lcainfohub/datasets/elcd/lciamethods/5296e2be-060b-4e50-b033-d45f85f6ac92.xml"}, "meanAmount": 0.0, "other": {"anies": [{"value": "0.78763664956648", "module": "A1", "scenario": "Standard scenario"}, {"value": "0.009222197", "module": "A2", "scenario": "Standard scenario"}, {"value": "0.044857543", "module": "A3", "scenario": "Standard scenario"}, {"value": "0.8417163895664801", "module": "A1-A3", "scenario": "Standard scenario"}, {"value": "0.003547376", "module": "A4", "scenario": "Standard scenario"}, {"value": "0.004981065", "module": "A5", "scenario": "Standard scenario"}, {"value": "4.76884E-4", "module": "C1", "scenario": "Standard scenario"}, {"value": "0.001586078", "module": "C2", "scenario": "Standard scenario"}, {"value": "0.007568933", "module": "C3", "scenario": "Standard scenario"}, {"value": "3.94464E-4", "module": "C4", "scenario": "Standard scenario"}, {"value": "-0.36413444", "module": "D", "scenario": "Standard scenario"}, {"name": "referenceToUnitGroupDataSet", "value": {"shortDescription": [{"value": "kg N eqv."}], "type": "unit group data set", "refObjectId": "d05bb823-ecdf-4686-8c40-bf1d9257859f", "uri": "../unitgroups/d05bb823-ecdf-4686-8c40-bf1d9257859f"}}]}}, {"referenceToLCIAMethodDataSet": {"shortDescription": [{"value": "Eutrophierungspotenzial - Land (EP-terrestrial)", "lang": "de"}, {"value": "Eutrophication potential - terrestrial (EP-terrestrial)", "lang": "en"}, {"value": "Övergödningspotential total (EP-T)", "lang": "sv"}], "type": "LCIA method data set", "refObjectId": "b5c614d2-def3-11e6-bf01-fe55135034f3", "version": "01.02.011", "uri": "http://lca.jrc.ec.europa.eu/lcainfohub/datasets/elcd/lciamethods/40054970-5936-477c-9bec-29fa23b1cb77.xml"}, "meanAmount": 0.0, "other": {"anies": [{"value": "8.71934100641399", "module": "A1", "scenario": "Standard scenario"}, {"value": "0.101675800671179", "module": "A2", "scenario": "Standard scenario"}, {"value": "0.496776364868385", "module": "A3", "scenario": "Standard scenario"}, {"value": "9.317793171953554", "module": "A1-A3", "scenario": "Standard scenario"}, {"value": "0.039713672", "module": "A4", "scenario": "Standard scenario"}, {"value": "0.056116711", "module": "A5", "scenario": "Standard scenario"}, {"value": "0.005876019", "module": "C1", "scenario": "Standard scenario"}, {"value": "0.017486692", "module": "C2", "scenario": "Standard scenario"}, {"value": "0.086235767", "module": "C3", "scenario": "Standard scenario"}, {"value": "0.003651085", "module": "C4", "scenario": "Standard scenario"}, {"value": "-4.146433716", "module": "D", "scenario": "Standard scenario"}, {"name": "referenceToUnitGroupDataSet", "value": {"shortDescription": [{"value": "mol N eqv."}], "type": "unit group data set", "refObjectId": "71b4d617-0ec9-4d3f-b65e-e438940c2401", "uri": "../unitgroups/71b4d617-0ec9-4d3f-b65e-e438940c2401"}}]}}, {"referenceToLCIAMethodDataSet": {"shortDescription": [{"value": "Globales Erwärmungspotenzial - total (GWP-total)", "lang": "de"}, {"value": "Global Warming Potential - total (GWP-total)", "lang": "en"}, {"value": "Global uppvärmningspotential – Totalt (GWP-T)", "lang": "sv"}], "type": "LCIA method data set", "refObjectId": "6a37f984-a4b3-458a-a20a-64418c145fa2", "version": "04.00.018"}, "meanAmount": 0.0, "other": {"anies": [{"value": "778.8098240924", "module": "A1", "scenario": "Standard scenario"}, {"value": "4.51626350231121", "module": "A2", "scenario": "Standard scenario"}, {"value": "0.279976059682049", "module": "A3", "scenario": "Standard scenario"}, {"value": "783.6060636543933", "module": "A1-A3", "scenario": "Standard scenario"}, {"value": "5.57107490104219", "module": "A4", "scenario": "Standard scenario"}, {"value": "45.410113132743", "module": "A5", "scenario": "Standard scenario"}, {"value": "0.664756452500541", "module": "C1", "scenario": "Standard scenario"}, {"value": "0.77672865125121", "module": "C2", "scenario": "Standard scenario"}, {"value": "18.7929322392399", "module": "C3", "scenario": "Standard scenario"}, {"value": "0.195047997174999", "module": "C4", "scenario": "Standard scenario"}, {"value": "-366.2753679", "module": "D", "scenario": "Standard scenario"}, {"name": "referenceToUnitGroupDataSet", "value": {"shortDescription": [{"value": "kg CO2-Äqv."}], "type": "unit group data set", "refObjectId": "1ebf3012-d0db-4de2-aefd-ef30cedb0be1", "uri": "../unitgroups/1ebf3012-d0db-4de2-aefd-ef30cedb0be1"}}]}}, {"referenceToLCIAMethodDataSet": {"shortDescription": [{"value": "Globales Erwärmungspotenzial - fossil (GWP-fossil)", "lang": "de"}, {"value": "Global Warming Potential - fossil fuels (GWP-fossil)", "lang": "en"}, {"value": "Global uppvärmningspotential– fossil (GWP-f)", "lang": "sv"}], "type": "LCIA method data set", "refObjectId": "5f635281-343e-44fb-83df-1971b155e6b6", "version": "01.00.011"}, "meanAmount": 0.0, "other": {"anies": [{"value": "773.355053217519", "module": "A1", "scenario": "Standard scenario"}, {"value": "4.51252675789662", "module": "A2", "scenario": "Standard scenario"}, {"value": "41.4971322603678", "module": "A3", "scenario": "Standard scenario"}, {"value": "819.3647122357834", "module": "A1-A3", "scenario": "Standard scenario"}, {"value": "5.56525874278765", "module": "A4", "scenario": "Standard scenario"}, {"value": "3.5108831462173", "module": "A5", "scenario": "Standard scenario"}, {"value": "0.643927696677244", "module": "C1", "scenario": "Standard scenario"}, {"value": "0.776085988030223", "module": "C2", "scenario": "Standard scenario"}, {"value": "18.4123545612599", "module": "C3", "scenario": "Standard scenario"}, {"value": "0.19430346345", "module": "C4", "scenario": "Standard scenario"}, {"value": "-366.6289867", "module": "D", "scenario": "Standard scenario"}, {"name": "referenceToUnitGroupDataSet", "value": {"shortDescription": [{"value": "kg CO2-Äqv."}], "type": "unit group data set", "refObjectId": "1ebf3012-d0db-4de2-aefd-ef30cedb0be1", "uri": "../unitgroups/1ebf3012-d0db-4de2-aefd-ef30cedb0be1"}}]}}, {"referenceToLCIAMethodDataSet": {"shortDescription": [{"value": "Globales Erwärmungspotenzial - biogen (GWP-biogenic)", "lang": "de"}, {"value": "Global Warming Potential - biogenic (GWP-biogenic)", "lang": "en"}, {"value": "Global uppvärmningspotential – biogen (GWP-b)", "lang": "sv"}], "type": "LCIA method data set", "refObjectId": "2356e1ab-0185-4db5-86e5-16de51c7485c", "version": "01.00.007"}, "meanAmount": 0.0, "other": {"anies": [{"value": "2.892968027437", "module": "A1", "scenario": "Standard scenario"}, {"value": "0.002083202", "module": "A2", "scenario": "Standard scenario"}, {"value": "-41.33432945", "module": "A3", "scenario": "Standard scenario"}, {"value": "-38.439278220563", "module": "A1-A3", "scenario": "Standard scenario"}, {"value": "0.003602206", "module": "A4", "scenario": "Standard scenario"}, {"value": "41.8973065742574", "module": "A5", "scenario": "Standard scenario"}, {"value": "0.019331248", "module": "C1", "scenario": "Standard scenario"}, {"value": "3.58279E-4", "module": "C2", "scenario": "Standard scenario"}, {"value": "0.375781833185075", "module": "C3", "scenario": "Standard scenario"}, {"value": "6.98609E-4", "module": "C4", "scenario": "Standard scenario"}, {"value": "1.6", "module": "D", "scenario": "Standard scenario"}, {"name": "referenceToUnitGroupDataSet", "value": {"shortDescription": [{"value": "kg CO2-Äqv."}], "type": "unit group data set", "refObjectId": "1ebf3012-d0db-4de2-aefd-ef30cedb0be1", "uri": "../unitgroups/1ebf3012-d0db-4de2-aefd-ef30cedb0be1"}}]}}, {"referenceToLCIAMethodDataSet": {"shortDescription": [{"value": "Globales Erwärmungspotenzial - luluc (GWP-luluc)", "lang": "de"}, {"value": "Global Warming Potential - land use and land use change (GWP-luluc)", "lang": "en"}, {"value": "Global uppvärmningspotential - markanvändning och förändringar i markanvändning (GWP-luluc)", "lang": "sv"}], "type": "LCIA method data set", "refObjectId": "4331bbdb-978a-490d-8707-eeb047f01a55", "version": "01.00.007"}, "meanAmount": 0.0, "other": {"anies": [{"value": "2.36961276708977", "module": "A1", "scenario": "Standard scenario"}, {"value": "0.001653542", "module": "A2", "scenario": "Standard scenario"}, {"value": "0.117123640822656", "module": "A3", "scenario": "Standard scenario"}, {"value": "2.4883899499124262", "module": "A1-A3", "scenario": "Standard scenario"}, {"value": "0.002213895", "module": "A4", "scenario": "Standard scenario"}, {"value": "0.001930453", "module": "A5", "scenario": "Standard scenario"}, {"value": "0.001497508", "module": "C1", "scenario": "Standard scenario"}, {"value": "2.84384E-4", "module": "C2", "scenario": "Standard scenario"}, {"value": "0.004845699", "module": "C3", "scenario": "Standard scenario"}, {"value": "4.37735E-5", "module": "C4", "scenario": "Standard scenario"}, {"value": "-1.382986583", "module": "D", "scenario": "Standard scenario"}, {"name": "referenceToUnitGroupDataSet", "value": {"shortDescription": [{"value": "kg CO2-Äqv."}], "type": "unit group data set", "refObjectId": "1ebf3012-d0db-4de2-aefd-ef30cedb0be1", "uri": "../unitgroups/1ebf3012-d0db-4de2-aefd-ef30cedb0be1"}}]}}, {"referenceToLCIAMethodDataSet": {"shortDescription": [{"value": "Abbaupotenzial der stratosphärischen Ozonschicht (ODP)", "lang": "de"}, {"value": "Depletion potential of the stratospheric ozone layer (ODP)", "lang": "en"}, {"value": "Utarmningspotential för stratosfäriska ozonskiktet - ozonnedbrytning (ODP)", "lang": "sv"}], "type": "LCIA method data set", "refObjectId": "b5c629d6-def3-11e6-bf01-fe55135034f3", "version": "02.00.014", "uri": "http://lca.jrc.ec.europa.eu/lcainfohub/datasets/elcd/lciamethods/8b723200-3d8f-4eec-9e10-444edb029476.xml"}, "meanAmount": 0.0, "other": {"anies": [{"value": "3.60258E-5", "module": "A1", "scenario": "Standard scenario"}, {"value": "9.96023E-7", "module": "A2", "scenario": "Standard scenario"}, {"value": "2.79781E-6", "module": "A3", "scenario": "Standard scenario"}, {"value": "3.9819633000000004E-5", "module": "A1-A3", "scenario": "Standard scenario"}, {"value": "1.30233E-6", "module": "A4", "scenario": "Standard scenario"}, {"value": "2.60506E-7", "module": "A5", "scenario": "Standard scenario"}, {"value": "5.42283E-8", "module": "C1", "scenario": "Standard scenario"}, {"value": "1.71301E-7", "module": "C2", "scenario": "Standard scenario"}, {"value": "7.75382E-7", "module": "C3", "scenario": "Standard scenario"}, {"value": "4.04791E-8", "module": "C4", "scenario": "Standard scenario"}, {"value": "-1.36198E-5", "module": "D", "scenario": "Standard scenario"}, {"name": "referenceToUnitGroupDataSet", "value": {"shortDescription": [{"value": "kg CFC 11-Äquiv."}], "type": "unit group data set", "refObjectId": "d9e957c9-7309-4474-bf3a-7777df6c4e5b", "uri": "../unitgroups/d9e957c9-7309-4474-bf3a-7777df6c4e5b"}}]}}, {"referenceToLCIAMethodDataSet": {"shortDescription": [{"value": "Bildungspotenzial für troposphärisches Ozon (POCP)", "lang": "de"}, {"value": "Photochemical Ozone Creation Potential (POCP)", "lang": "en"}, {"value": "Potential till fotokemisk oxidantbildning – marknära ozon (POCP)", "lang": "sv"}], "type": "LCIA method data set", "refObjectId": "b5c610fe-def3-11e6-bf01-fe55135034f3", "version": "02.00.018", "uri": "http://lca.jrc.ec.europa.eu/lcainfohub/datasets/elcd/lciamethods/ec7836be-83eb-41da-bcda-1a6a3fe2d149.xml"}, "meanAmount": 0.0, "other": {"anies": [{"value": "2.52558743636839", "module": "A1", "scenario": "Standard scenario"}, {"value": "0.029029173", "module": "A2", "scenario": "Standard scenario"}, {"value": "0.164609896660338", "module": "A3", "scenario": "Standard scenario"}, {"value": "2.719226506028728", "module": "A1-A3", "scenario": "Standard scenario"}, {"value": "0.015499668", "module": "A4", "scenario": "Standard scenario"}, {"value": "0.014999909", "module": "A5", "scenario": "Standard scenario"}, {"value": "0.001491053", "module": "C1", "scenario": "Standard scenario"}, {"value": "0.004992576", "module": "C2", "scenario": "Standard scenario"}, {"value": "0.023950037", "module": "C3", "scenario": "Standard scenario"}, {"value": "0.001070277", "module": "C4", "scenario": "Standard scenario"}, {"value": "-1.202419455", "module": "D", "scenario": "Standard scenario"}, {"name": "referenceToUnitGroupDataSet", "value": {"shortDescription": [{"value": "kg NMVOC eqv."}], "type": "unit group data set", "refObjectId": "d27c25f8-fbc1-44c6-b47b-4adbae4199c6", "uri": "../unitgroups/d27c25f8-fbc1-44c6-b47b-4adbae4199c6"}}]}}, {"referenceToLCIAMethodDataSet": {"shortDescription": [{"value": "Wasser-Entzugspotenzial (Benutzer) (WDP)", "lang": "de"}, {"value": "Water (user) deprivation potential (WDP)", "lang": "en"}, {"value": "Vattenfotavtryck (WDP)", "lang": "sv"}], "type": "LCIA method data set", "refObjectId": "b2ad66ce-c78d-11e6-9d9d-cec0c932ce01", "version": "03.00.016"}, "meanAmount": 0.0, "other": {"anies": [{"value": "131.75342372994", "module": "A1", "scenario": "Standard scenario"}, {"value": "0.243490341566103", "module": "A2", "scenario": "Standard scenario"}, {"value": "11.6529962707928", "module": "A3", "scenario": "Standard scenario"}, {"value": "143.64991034229894", "module": "A1-A3", "scenario": "Standard scenario"}, {"value": "0.293968152547066", "module": "A4", "scenario": "Standard scenario"}, {"value": "0.382029635052603", "module": "A5", "scenario": "Standard scenario"}, {"value": "0.14841471082477", "module": "C1", "scenario": "Standard scenario"}, {"value": "0.041876636", "module": "C2", "scenario": "Standard scenario"}, {"value": "1.0715725037965", "module": "C3", "scenario": "Standard scenario"}, {"value": "0.041360831", "module": "C4", "scenario": "Standard scenario"}, {"value": "-27.60451412", "module": "D", "scenario": "Standard scenario"}, {"name": "referenceToUnitGroupDataSet", "value": {"shortDescription": [{"value": "m3 world eqv."}], "type": "unit group data set", "refObjectId": "6ae2df01-888e-46c8-b17d-49fa3869b476", "uri": "../unitgroups/6ae2df01-888e-46c8-b17d-49fa3869b476"}}]}}, {"referenceToLCIAMethodDataSet": {"shortDescription": [{"value": "Potenzielles Auftreten von Krankheiten aufgrund von Feinstaubemissionen (PM)", "lang": "de"}, {"value": "Potential incidence of disease due to PM emissions (PM)", "lang": "en"}, {"value": "Potential till utsläpp av partiklar (PM)", "lang": "sv"}], "type": "LCIA method data set", "refObjectId": "b5c602c6-def3-11e6-bf01-fe55135034f3", "version": "02.00.013", "uri": "http://lca.jrc.ec.europa.eu/lcainfohub/datasets/elcd/lciamethods/72ce3013-f678-4c6a-935b-f4752ff8901b.xml"}, "meanAmount": 0.0, "other": {"anies": [{"value": "6.05529E-5", "module": "A1", "scenario": "Standard scenario"}, {"value": "4.05963E-7", "module": "A2", "scenario": "Standard scenario"}, {"value": "3.15652E-6", "module": "A3", "scenario": "Standard scenario"}, {"value": "6.4115383E-5", "module": "A1-A3", "scenario": "Standard scenario"}, {"value": "4.05426E-7", "module": "A4", "scenario": "Standard scenario"}, {"value": "1.19258E-7", "module": "A5", "scenario": "Standard scenario"}, {"value": "9.8391E-9", "module": "C1", "scenario": "Standard scenario"}, {"value": "6.98195E-8", "module": "C2", "scenario": "Standard scenario"}, {"value": "4.75828E-7", "module": "C3", "scenario": "Standard scenario"}, {"value": "1.87995E-8", "module": "C4", "scenario": "Standard scenario"}, {"value": "-2.89239E-5", "module": "D", "scenario": "Standard scenario"}, {"name": "referenceToUnitGroupDataSet", "value": {"shortDescription": [{"value": "disease incidence"}], "type": "unit group data set", "refObjectId": "3883559b-648f-4afc-8ba2-0bd24f3affa3", "uri": "../unitgroups/3883559b-648f-4afc-8ba2-0bd24f3affa3"}}]}}, {"referenceToLCIAMethodDataSet": {"shortDescription": [{"value": "Potenzielle Wirkung durch Exposition des Menschen mit U235 (IRP)", "lang": "de"}, {"value": "Potential Human exposure efficiency relative to U235 (IRP)", "lang": "en"}, {"value": "Exponeringseffektivitet relaterad till U235 (IR)", "lang": "sv"}], "type": "LCIA method data set", "refObjectId": "b5c632be-def3-11e6-bf01-fe55135034f3", "version": "01.00.013", "uri": "http://lca.jrc.ec.europa.eu/lcainfohub/datasets/elcd/lciamethods/a6f4cbc8-5388-44d6-9a67-53d05684f93e.xml"}, "meanAmount": 0.0, "other": {"anies": [{"value": "16.2193686766314", "module": "A1", "scenario": "Standard scenario"}, {"value": "0.285152592171734", "module": "A2", "scenario": "Standard scenario"}, {"value": "1.39907617211093", "module": "A3", "scenario": "Standard scenario"}, {"value": "17.903597440914066", "module": "A1-A3", "scenario": "Standard scenario"}, {"value": "0.3824168235828", "module": "A4", "scenario": "Standard scenario"}, {"value": "0.161283130543362", "module": "A5", "scenario": "Standard scenario"}, {"value": "0.114499068148114", "module": "C1", "scenario": "Standard scenario"}, {"value": "0.04904191", "module": "C2", "scenario": "Standard scenario"}, {"value": "0.297112103553775", "module": "C3", "scenario": "Standard scenario"}, {"value": "0.012049261", "module": "C4", "scenario": "Standard scenario"}, {"value": "-4.550546135", "module": "D", "scenario": "Standard scenario"}, {"name": "referenceToUnitGroupDataSet", "value": {"shortDescription": [{"value": "kBq U235 eqv."}], "type": "unit group data set", "refObjectId": "456b05bf-1415-44a9-9993-02452f554c09", "uri": "../unitgroups/456b05bf-1415-44a9-9993-02452f554c09"}}]}}, {"referenceToLCIAMethodDataSet": {"shortDescription": [{"value": "Potenzielle Toxizitätsvergleichseinheit für Ökosysteme (ETP-fw)", "lang": "de"}, {"value": "Potential Comparative Toxic Unit for ecosystems (ETP-fw)", "lang": "en"}, {"value": "Ecotoxicitet (ETP-fw) ", "lang": "sv"}], "type": "LCIA method data set", "refObjectId": "ee1082d1-b0f7-43ca-a1f0-21e2a4a74511", "version": "01.00.004", "uri": "http://lca.jrc.ec.europa.eu/lcainfohub/datasets/elcd/lciamethods/ee1082d1-b0f7-43ca-a1f0-21e2a4a74511.xml"}, "meanAmount": 0.0, "other": {"anies": [{"value": "19840.07", "module": "A1", "scenario": "Standard scenario"}, {"value": "60.6886541786734", "module": "A2", "scenario": "Standard scenario"}, {"value": "1132.51", "module": "A3", "scenario": "Standard scenario"}, {"value": "21033.26865417867", "module": "A1-A3", "scenario": "Standard scenario"}, {"value": "73.219252950718", "module": "A4", "scenario": "Standard scenario"}, {"value": "48.0359773472852", "module": "A5", "scenario": "Standard scenario"}, {"value": "9.07275817843663", "module": "C1", "scenario": "Standard scenario"}, {"value": "10.4375257294727", "module": "C2", "scenario": "Standard scenario"}, {"value": "401.58367798535", "module": "C3", "scenario": "Standard scenario"}, {"value": "400.28771540495", "module": "C4", "scenario": "Standard scenario"}, {"value": "-9030.24", "module": "D", "scenario": "Standard scenario"}, {"name": "referenceToUnitGroupDataSet", "value": {"shortDescription": [{"value": "CTUe"}], "type": "unit group data set", "refObjectId": "aa959ded-f1eb-4efb-9c5c-2d60be36b3e6", "uri": "../unitgroups/aa959ded-f1eb-4efb-9c5c-2d60be36b3e6"}}]}}, {"referenceToLCIAMethodDataSet": {"shortDescription": [{"value": "Potenzielle Toxizitätsvergleichseinheit für den Menschen - kanzerogene Wirkung (HTP-c)", "lang": "de"}, {"value": "Potential Comparative Toxic Unit for humans - cancer effects (HTP-c)", "lang": "en"}, {"value": "Humantoxicitet – cancer (HTP-c)", "lang": "sv"}], "type": "LCIA method data set", "refObjectId": "2299222a-bbd8-474f-9d4f-4dd1f18aea7c", "version": "01.00.005", "uri": "http://lca.jrc.ec.europa.eu/lcainfohub/datasets/elcd/lciamethods/2299222a-bbd8-474f-9d4f-4dd1f18aea7c.xml"}, "meanAmount": 0.0, "other": {"anies": [{"value": "4.00871E-6", "module": "A1", "scenario": "Standard scenario"}, {"value": "1.9684E-9", "module": "A2", "scenario": "Standard scenario"}, {"value": "6.28314E-8", "module": "A3", "scenario": "Standard scenario"}, {"value": "4.0735098E-6", "module": "A1-A3", "scenario": "Standard scenario"}, {"value": "2.0666E-9", "module": "A4", "scenario": "Standard scenario"}, {"value": "7.12841E-9", "module": "A5", "scenario": "Standard scenario"}, {"value": "2.34264E-10", "module": "C1", "scenario": "Standard scenario"}, {"value": "3.38535E-10", "module": "C2", "scenario": "Standard scenario"}, {"value": "7.27224E-9", "module": "C3", "scenario": "Standard scenario"}, {"value": "5.83305E-11", "module": "C4", "scenario": "Standard scenario"}, {"value": "-4.92078E-7", "module": "D", "scenario": "Standard scenario"}, {"name": "referenceToUnitGroupDataSet", "value": {"shortDescription": [{"value": "CTUh"}], "type": "unit group data set", "refObjectId": "d4c9523e-2d7e-49fd-8469-998f547d3a70", "uri": "../unitgroups/d4c9523e-2d7e-49fd-8469-998f547d3a70"}}]}}, {"referenceToLCIAMethodDataSet": {"shortDescription": [{"value": "Potenzielle Toxizitätsvergleichseinheit für den Menschen - nicht kanzerogene Wirkung (HTP-nc)", "lang": "de"}, {"value": "Potential Comparative Toxic Unit for humans - non-cancer effects (HTP-nc)", "lang": "en"}, {"value": "Humantoxicitet – icke cancer (HTP-nc)", "lang": "sv"}], "type": "LCIA method data set", "refObjectId": "3af763a5-b7a1-48c9-9cee-1f223481fcef", "version": "01.00.004", "uri": "http://lca.jrc.ec.europa.eu/lcainfohub/datasets/elcd/lciamethods/3af763a5-b7a1-48c9-9cee-1f223481fcef.xml"}, "meanAmount": 0.0, "other": {"anies": [{"value": "1.81942E-5", "module": "A1", "scenario": "Standard scenario"}, {"value": "6.63843E-8", "module": "A2", "scenario": "Standard scenario"}, {"value": "9.18136E-7", "module": "A3", "scenario": "Standard scenario"}, {"value": "1.91787203E-5", "module": "A1-A3", "scenario": "Standard scenario"}, {"value": "7.75163E-8", "module": "A4", "scenario": "Standard scenario"}, {"value": "4.41022E-8", "module": "A5", "scenario": "Standard scenario"}, {"value": "7.98826E-9", "module": "C1", "scenario": "Standard scenario"}, {"value": "1.14171E-8", "module": "C2", "scenario": "Standard scenario"}, {"value": "2.96409E-7", "module": "C3", "scenario": "Standard scenario"}, {"value": "1.79275E-9", "module": "C4", "scenario": "Standard scenario"}, {"value": "-7.27486E-6", "module": "D", "scenario": "Standard scenario"}, {"name": "referenceToUnitGroupDataSet", "value": {"shortDescription": [{"value": "CTUh"}], "type": "unit group data set", "refObjectId": "d4c9523e-2d7e-49fd-8469-998f547d3a70", "uri": "../unitgroups/d4c9523e-2d7e-49fd-8469-998f547d3a70"}}]}}, {"referenceToLCIAMethodDataSet": {"shortDescription": [{"value": "Potenzieller Bodenqualitätsindex (SQP)", "lang": "de"}, {"value": "Potential Soil quality index (SQP)", "lang": "en"}, {"value": "Potentiell jordkvalitet index (SQP)", "lang": "sv"}], "type": "LCIA method data set", "refObjectId": "b2ad6890-c78d-11e6-9d9d-cec0c932ce01", "version": "01.00.014"}, "meanAmount": 0.0, "other": {"anies": [{"value": "1931.65", "module": "A1", "scenario": "Standard scenario"}, {"value": "59.0226783769366", "module": "A2", "scenario": "Standard scenario"}, {"value": "5236.8", "module": "A3", "scenario": "Standard scenario"}, {"value": "7227.4726783769365", "module": "A1-A3", "scenario": "Standard scenario"}, {"value": "80.3675558741465", "module": "A4", "scenario": "Standard scenario"}, {"value": "12.4252885283057", "module": "A5", "scenario": "Standard scenario"}, {"value": "3.23564985807184", "module": "C1", "scenario": "Standard scenario"}, {"value": "10.1510032232376", "module": "C2", "scenario": "Standard scenario"}, {"value": "63.422460541275", "module": "C3", "scenario": "Standard scenario"}, {"value": "6.00874599194999", "module": "C4", "scenario": "Standard scenario"}, {"value": "-2157.12", "module": "D", "scenario": "Standard scenario"}, {"name": "referenceToUnitGroupDataSet", "value": {"shortDescription": [{"value": "dimensionless"}], "type": "unit group data set", "refObjectId": "f130951c-e67f-4f7f-8dd4-665de3974e18", "uri": "../unitgroups/f130951c-e67f-4f7f-8dd4-665de3974e18"}}]}}]}, "otherAttributes": {"{http://www.okworx.com/ILCD/Extensions/2018/Profile}profile": "EN_15804_A2", "{http://www.indata.network/EPD/2019}epd-version": "1.2"}, "version": "1.1"}