{"processInformation": {"dataSetInformation": {"UUID": "2556af6f-0e61-42f4-9bca-8bd35c7521e0", "name": {"baseName": [{"value": "Badewannen, Duschwannen und Wannenverkleidungen aus Acryl", "lang": "de"}, {"value": "Acrylic bathtubs, shower trays and bath panels", "lang": "en"}], "functionalUnitFlowProperties": [{"lang": "de"}]}, "classificationInformation": {"classification": [{"class": [{"value": "Gebäudetechnik", "level": 0, "classId": "8"}, {"value": "Sanitär", "level": 1, "classId": "8.3"}, {"value": "Dusch- und Badewannen", "level": 2, "classId": "8.3.03"}], "name": "OEKOBAU.DAT"}, {"class": [{"value": "03 Gebäudetechnik", "level": 0}, {"value": "Sanitäreinrichtungen", "level": 1}, {"value": "Sanitärprodukte aus Verbundwerkstoffen", "level": 2}], "name": "IBUCategories"}]}, "generalComment": [{"value": "Das durchschnittliche Acrylsanitärprodukt wird aus einer Produktgruppe abgeleitet, die Bade- und Duschwannen sowie Verkleidungen für Wannen umfasst. Die in der Acrylherstellung verwendeten Ausgangsstoffe sind Acrylplatten (PMMA –  Poly-methylmethacrylat), Kunstharz (Polyesterharz), Glasfaser, Calciumcarbonat und Holz. Für diese Studie wurde ein Acryl-Durchschnittsprodukt aus der produzierten Gesamtmasse an Acrylprodukten der im Referenzjahr 2019 betrachteten Gruppe gebildet.", "lang": "de"}, {"value": "The average sanitary acrylic product derives from a group of products including bathtubs, shower trays and bath panels. Materials involved in acrylic production are acrylic sheets (PMMA - polymethyl methacrylate), synthetic resin (polyester resin), glass fibre, calcium carbonate and wood. Particularly, the study focuses on the average acrylic product resulting from the total mass produced for the acrylic products of the considered group in the reference year 2019.Bathtubs are made of a thermoformed acrylic base body which is enhanced with the help of wood and a fiberglass-resin mixture from the bottom.", "lang": "en"}]}, "quantitativeReference": {"referenceToReferenceFlow": [0]}, "time": {"referenceYear": 2021, "dataSetValidUntil": 2026, "other": {"anies": [{"name": "publicationDateOfEPD", "value": 1639958400000}]}}, "geography": {"locationOfOperationSupplyOrProduction": {"location": "GLO"}}, "technology": {"technologyDescriptionAndIncludedProcesses": [{"value": "Die Acrylplatten (PMMA) werden zunächst von Staub und anderen Fremdpartikeln befreit, zugeschnitten und anschließend in einem Elektroofen bei 180 °C erhitzt, um in eine vorgeformte Form tiefgezogen zu werden. Nach dem Abkühlen wird die Acrylform mit einem Gemisch aus Polyesterharz, Glasfaser, Aceton und Calciumcarbonat besprüht. Weitere Komponenten des Gemischs für die Polymerisation sind Methylethylketonperoxid (Katalysator), Titandioxid (Pigment) und Cobalt (Aushärtungsbeschleuniger). Eine zusätzliche Schicht aus Holzplatten, die mit einem Gemisch aus Polyesterharz und Glasfaser besprüht werden, sorgt für Stabilität. Diese Schicht wird anschließend verdichtet. Nach dem Aushärten wird das Endprodukt der abschließenden Fertigungs-stufe zugeführt: (i) Überflüssige Kanten werden abgeschnitten und geschliffen und (ii) Öffnungen für Ablaufventile und sonstiges Zubehör werden angebracht. Die Produkte werden überwiegend in Folie und Karton verpackt und mit Stretchfolie auf den Paletten befestigt. Die überwiegend aus Polyesterharz, Glasfaser, Epoxidharz und Metall bestehenden Formen zum Thermoformen der erwärmten Acryl-platten werden ebenfalls im Werk in Kairo hergestellt, das nach ISO 9001 zertifiziert ist. \nTechnische Daten: \nBade- und Duschwannen von Duravit erfüllen je nach Modell, verwendetem Installationszubehör sowie baulicher Situation einzelne oder mehrere Schall-schutznormen. Hierzu zählen: DIN 4109 (A1), VDI 4100, SIA 181.\n Die Abmessungen der Produkte bei der Lieferung sind in der folgenden Tabelle aufgelistet und werden mit Länge (L), Breite (B) und Höhe (H) angegeben. Weitere technische Daten sind für die Gruppe der Acrylsanitärprodukte im Rahmen dieser Studie nicht relevant. \nDeklarierte Einheit: \nFür die Berechnung der Ökobilanz wird eine deklarierte Einheit von 1 m² Acryl-Oberfläche eines Durchschnittsprodukts aus Bade- und Duschwannen sowie Wannenverkleidungen zugrunde gelegt. Alle Umweltauswirkungen des Produkts werden auf 1 m² Acryl-Oberfläche bezogen. Aufgrund der identischen Herstellungsweise wird ein Durchschnittsprodukt aus Bade- und Duschwannen sowie aus Wannenver-kleidungen auf Basis der Gesamtproduktionsmengen der jeweiligen Acrylprodukte im Betrachtungsjahr 2019 gebildet. Zubehörteile für die Produkte werden innerhalb dieser Studie nicht betrachtet, da die Analyse von elektronischen Komponenten und Düsen für Badewannensysteme den Rahmen dieser Studie übersteigen würde. Darüber hinaus finden sonstiges Zubehör wie Füße und Fußsysteme bei den betrachteten Produkten kaum Anwendung.  \n\nDie Schichtdicke der Acrylfläche kann folgendermaßen für die jeweiligen Produkte unterschieden werden:\n\nBadewannen: 4–5 mm\nDuschwannen: 3,2–4 mm\nVerkleidungen: 4–5 mm\n\n\nDie Dichte von PMMA-Platten wird in der Literatur mit 1190 kg/m³ angegeben. Daraus ergibt sich ein Gewicht des Durchschnittsprodukts (ohne Verpackung) von 17,91 kg pro deklarierte Einheit (1 m²). Für die Verpackung wird ein Gewicht von 0,21 kg pro deklarierte Einheit definiert*. \n\n*Zu weiteren technischen Angaben (z. B. spezielle Abmessungen und Gewichtsangaben) zu den einzelnen Produkten (Bade- und Duschwannen sowie Verkleidungen), die das Durchschnittsprodukt bilden, siehe: \n\nhttps://pro.duravit.de/pro/content/homepage/produkte/kategorien/uebersicht~402880943a1b6e1b013a1bd065b4001f.de-de.html?categories= Zur Umrechnung der Produktmasse (kg) in die äquivalente Oberfläche (m2) ist der Massewert mit dem in der Tabelle unten angegebenen Umrechnungsfaktor zu multiplizieren (0,055).", "lang": "de"}, {"value": "After the acrylic (PMMA) sheets have been delivered, they are first cleaned freed of dust and other foreign particles, cut to size and then thermoformed in an electrically powered oven at 180°C to be drawn into a preformed shape. After the cooling phase, carried out mainly by fans, the acrylic mould is sprayed all around with a mixture of polyester resin, glass fibre, acetone and calcium carbonate. Additional components of the mixture for polymerization are methyl ethyl ketone peroxide (catalyst), titanium dioxide (pigment) and cobalt (hardening accelerator). In order to improve the stability of the product, there is an additional layer of wood panels on the flat areas of the product (rim and stand area), which is then sprayed again with the polyester resin-glass fibre mixture. With the help of manual processing in the form of rollers, the mixture is compressed and then passes through the curing tunnel for the curing process. Once curing is complete, product is subjected to finishing stage which consists mainly of two processes: on the one hand, unnecessary edges are cut and smoothed, and on the other hand, holes are drilled for waste valve and other accessories (like overflow or handleswhich which are not part of the present study). The products are packed in film and cardboard, which are then fixed to the pallets with stretch film. Some products are also protected against transport damage with wood and foam. The moulds for the deep drawing of the heated acrylic sheets are also produced at the Cairo site and are included in the calculation. The moulds are mainly made of polyester resin, fiberglass, epoxy resin and metal. \nTechnical data: \nDepending on the model, installation accessories used and the respective structural situation, bathtubs and shower trays by Duravit fulfil individual or several sound insulation standards. These include: DIN 4109 (A1), VDI 4100, SIA 181.\n The product dimensions on delivery are listed in the following table according to length (L), width (W) and height (H). No other technical data is of relevance for the sanitary acrylic product group object of the study. \nDeclared unit: \nA declared unit of 1 m² of acrylic surface of an average product including bathtubs and shower trays, as well as acrylic panels, is used as the basis for calculating the life cycle assessment. All environmental impacts of the product are related to 1 m² of acrylic surface. Because of the identical manufacturing method, an average acrylic product made of bathtubs and shower trays, as well as acrylic panels, has been considered according to the total mass produced for the respective acrylic products for the reference year 2019. Product accessories are not considered within this study since the analysis of elements such as electronic parts and nozzles for bathtub systems would be beyond the scope of this study. Moreover, other accessories like feet and foot systems are also excluded since the are almost avoided in the products under study. \n\nThe thickness of the acrylic surface coating can be distinguished as follows for the respective products: \nBathtubs: 4 - 5 mm \nShower trays: 3.2 - 4 mm \nPanels: 4 - 5 mm\n\nThe density of PMMA plates is indicated in the literature as 1190 kg/m³ , resulting in an average product weight (without packaging) equal to 17.91 kg per declared unit (1 m²). The packaging is defined with a weight of 0.21 kg per declared unit*.*Additional technical information (i.e. specific dimensions and weight) about each (every) single product (bathtubs, shower trays and bath panels) making the average product are available at:\n\n https://pro.duravit.de/pro/content/homepage/produkte/kategorien/uebersicht~402880943a1b6e1b013a1bd065b4001f.de-de.html?categories=\n\nThe conversion from mass (kg) of product to the equivalent surface (m2) needs to be performed multiplying the mass value by the conversion factor highlighted in the below table (0.055).", "lang": "en"}], "technologicalApplicability": [{"value": "Die Gruppe der Acrylsanitärprodukte umfasst Badewannen, Duschwannen und Wannenver-kleidungen zur Verwendung in Bädern. Bade- und Duschwannen sind Einrichtungsgegenstände für Badezimmer und werden insbesondere für die Körperhygiene genutzt. Wannenverkleidungen sind als Zubehör für Badewannen erhältlich.", "lang": "de"}, {"value": "The sanitary acrylic group includes bathtubs, shower trays and bath panels used in bathrooms. Bathtubs and shower trays are furnishings for bathrooms, which are used in particular for personal hygiene. Bath panels, instead, is used as an accessory for bathtubs.", "lang": "en"}]}}, "modellingAndValidation": {"LCIMethodAndAllocation": {"typeOfDataSet": "EPD", "referenceToLCAMethodDetails": [{"shortDescription": [{"value": "Sanitärprodukte aus Verbundwerkstoffen.pdf", "lang": "de"}], "type": "source data set", "refObjectId": "1981f3cc-9fe5-4e67-89de-1cb37a5b5a95"}], "other": {"anies": [{"name": "subType", "value": "average dataset"}]}}, "dataSourcesTreatmentAndRepresentativeness": {"referenceToDataSource": [{"shortDescription": [{"value": "ecoinvent database (all versions)", "lang": "de"}], "type": "source data set", "refObjectId": "b497a91f-e14b-4b69-8f28-f50eb1576766"}, {"shortDescription": [{"value": "ecoinvent 3.6 database", "lang": "de"}], "type": "source data set", "refObjectId": "766b9973-5ee8-48a2-8098-72c8e20b369f"}], "useAdviceForDataSet": [{"value": "Gültigkeitsbereich: \nGegenstand der vorliegenden Studie ist die Erstellung einer Ökobilanz für Acrylsanitärprodukte von Duravit inklusive Verpackung, produziert am Standort Kairo in Ägypten und weltweit vertrieben. Grundlage für die Datenerhebung ist das Jahr 2019. Aufgrund der identischen Herstellungsweise wird im Rahmen dieser EPD die durchschnittliche Produktion des Werks von Acrylerzeugnissen, d. h. Bade- und Duschwannen sowie Wannenverkleidungen, unter Berücksichtigung der produzierten Gesamtmenge der jeweiligen Acrylprodukte im Referenzjahr 2019 betrachtet. Die Systemgrenzen umfassen die Module A1–A3, C1–C4 und D gemäß den Anforderungen der Referenznorm EN 15804+A2:2019 nach dem Ansatz „Von der Wiege bis zum Werkstor mit den Modulen C1–C4 und Modul D“. \nSystemgrenze: \nDie Systemgrenzen umfassen die Module A1–A3, C1–C4 und D gemäß dem Ansatz „von der Wiege bis zum Werkstor mit den Modulen C1–C4 und Modul D“. Errichtung, Wartung und Abriss von Infrastruktur (mit Bezug auf Gebäude) sowie die Nutzung von Industrie-gelände werden in dieser Bewertung nicht berück-sichtigt, da ihr Beitrag vernachlässigbar ist. Darüber sind das Stadium der Errichtung des Bauwerks (Module A4–A5) und das Nutzungsstadium (Module B1–B7) nicht Gegenstand dieser Bewertung. Insbesondere aufgrund des bewerteten Produkttyps sind die Ergebnisse für C1 und C3 gleich null.", "lang": "de"}, {"value": "Scope: \nThis study is aimed to provide the life cycle impact assessment of Duravit sanitary acrylic products, including packaging, produced at Cairo plant in Egypt and distributed worldwide. The basis for the data collection is the year 2019. Due to the identical production method, the object of the EPD is the average acrylic production of the whole plant including bathtubs and shower trays, as well as acrylic panels, considering the total mass produced for the respective acrylic products for the reference year 2019. The system boundaries include the module A1-A3, C1-C4 and D, according to the requirements of the reference standard EN 15804+A2:2019, with an approach “from cradle to gate with modules C1–C4 and module D”. \nSystem boundary: \nThe system boundaries include the module A1-A3, C1-C4 and D with an approach “from cradle to gate with modules C1–C4 and module D”. Construction, maintenance and decommissioning of infrastructures (in terms of buildings) and the occupation of industrial land are not part of the assessment since their contribution is negligible. Moreover, construction process stage (modules A4-A5) and use phase (modules B1-B7) are not included in the assessment. Particularly, because of the type of product assessed, C1 and C3 results both equal to zero.", "lang": "en"}], "other": {"anies": [{"name": "referenceToOriginalEPD", "value": {"shortDescription": {"value": "Badewannen, Duschwannen und Wannenverkleidungen aus Acryl.pdf", "defaultValue": "Badewannen, Duschwannen und Wannenverkleidungen aus Acryl.pdf", "lstrings": [{"lang": "de", "value": "Badewannen, Duschwannen und Wannenverkleidungen aus Acryl.pdf"}]}, "type": "source data set", "uuid": {"uuid": "5515854d-f482-47ea-ab6c-cc57e3e1ae04"}, "refObjectId": "5515854d-f482-47ea-ab6c-cc57e3e1ae04", "resourceURLs": ["https://oekobaudat.de/OEKOBAU.DAT/resource/sources/5515854d-f482-47ea-ab6c-cc57e3e1ae04/Badewannen_Duschwannen_und_Wannenverkleidungen_aus_Acryl_19581.pdf?version=00.03.000"]}}]}}, "validation": {"review": [{"referenceToNameOfReviewerAndInstitution": [{"shortDescription": [{"value": "Institut Bauen und Umwelt e. V.", "lang": "de"}], "type": "contact data set", "refObjectId": "d111dbec-b024-4be5-86c5-752d6eb2cf95", "uri": "../contacts/d111dbec-b024-4be5-86c5-752d6eb2cf95.xml"}], "type": "Accredited third party review"}]}, "complianceDeclarations": {"compliance": [{"referenceToComplianceSystem": {"shortDescription": [{"value": "DIN EN 15804+A2", "lang": "de"}], "type": "source data set", "refObjectId": "c0016b33-8cf7-415c-ac6e-deba0d21440d", "uri": "../sources/c0016b33-8cf7-415c-ac6e-deba0d21440d.xml"}}, {"referenceToComplianceSystem": {"shortDescription": [{"value": "ISO 14025", "lang": "de"}], "type": "source data set", "refObjectId": "4f2eb655-6e44-4874-a95a-e28f5442cd4d", "uri": "../sources/4f2eb655-6e44-4874-a95a-e28f5442cd4d.xml"}}]}}, "administrativeInformation": {"commissionerAndGoal": {"referenceToCommissioner": [{"shortDescription": [{"value": "DURAVIT AG", "lang": "de"}], "type": "contact data set", "refObjectId": "0ab2b967-3743-4bbc-9f89-23e6406e6ab5", "uri": "../contacts/0ab2b967-3743-4bbc-9f89-23e6406e6ab5.xml"}]}, "dataGenerator": {"referenceToPersonOrEntityGeneratingTheDataSet": [{"shortDescription": [{"value": "SGS-TÜV Saar GmbH", "lang": "de"}], "type": "contact data set", "refObjectId": "9a1039cf-7187-4eb5-ae54-000c43ddb648", "uri": "../contacts/9a1039cf-7187-4eb5-ae54-000c43ddb648.xml"}]}, "dataEntryBy": {"timeStamp": 1639958400000, "referenceToDataSetFormat": [{"shortDescription": [{"value": "ILCD Format", "lang": "de"}], "type": "source data set", "refObjectId": "a97a0155-0234-4b87-b4ce-a45da52f2a40", "uri": "../sources/a97a0155-0234-4b87-b4ce-a45da52f2a40.xml"}, {"shortDescription": [{"value": "EPD-Datenformaterweiterungen v1.2", "lang": "de"}, {"value": "EPD Data Format Extensions v1.2", "lang": "en"}], "type": "source data set", "refObjectId": "a29449fd-aa2f-4de8-b5d7-4b06b43c6fde", "uri": "../sources/a29449fd-aa2f-4de8-b5d7-4b06b43c6fde.xml"}]}, "publicationAndOwnership": {"dataSetVersion": "00.02.000", "referenceToRegistrationAuthority": {"shortDescription": [{"value": "Institut Bauen und Umwelt e. V.", "lang": "de"}], "type": "contact data set", "refObjectId": "d111dbec-b024-4be5-86c5-752d6eb2cf95", "uri": "../contacts/d111dbec-b024-4be5-86c5-752d6eb2cf95.xml"}, "registrationNumber": "EPD-DUR-20210239-IBC1-DE", "referenceToOwnershipOfDataSet": {"shortDescription": [{"value": "DURAVIT AG", "lang": "de"}], "type": "contact data set", "refObjectId": "0ab2b967-3743-4bbc-9f89-23e6406e6ab5", "uri": "../contacts/0ab2b967-3743-4bbc-9f89-23e6406e6ab5.xml"}, "copyright": true, "licenseType": "Free of charge for all users and uses", "accessRestrictions": [{"value": "None", "lang": "en"}], "other": {"anies": [{"name": "referenceToPublisher", "value": {"shortDescription": [{"value": "Institut Bauen und Umwelt e. V.", "lang": "de"}], "type": "contact data set", "refObjectId": "d111dbec-b024-4be5-86c5-752d6eb2cf95", "uri": "../contacts/d111dbec-b024-4be5-86c5-752d6eb2cf95.xml"}}]}}}, "exchanges": {"exchange": [{"dataSetInternalID": 0, "referenceToFlowDataSet": {"shortDescription": [{"value": "1 m² Acryloberfläche eines durchschnittlichen Produkts, einschließlich Badewannen, Duschwannen und Acrylplatten (1 m² Acryloberfläche eines durchschnittlichen Produkts, einschließlich Badewannen, Duschwannen und Acrylplatten)", "lang": "de"}], "type": "flow data set", "refObjectId": "3c6e11dc-5754-81d5-02a4-9d5557c580b4", "uri": "../flows/3c6e11dc-5754-81d5-02a4-9d5557c580b4.xml"}, "meanAmount": 1.0, "referencesToDataSource": {}, "referenceFlow": true, "resolvedFlowVersion": "00.02.000", "resultingflowAmount": 1.0, "flowProperties": [{"name": [{"lang": "en", "value": "Area"}, {"lang": "de", "value": "Fläche"}], "uuid": "93a60a56-a3c8-19da-a746-0800200c9a66", "referenceFlowProperty": true, "meanValue": 1.0, "referenceUnit": "qm", "unitGroupUUID": "c20a03d7-bd90-4569-bc94-66cfd364dfc8"}, {"name": [{"lang": "de", "value": "Gewicht"}], "uuid": "93a60a56-a3c8-11da-a746-0800200b9a66", "meanValue": 17.91}], "materialProperties": [{"name": "layer thickness", "value": "0.004", "unit": "m", "unitDescription": "meters"}, {"name": "grammage", "value": "17.91", "unit": "kg/m^2", "unitDescription": "kilograms per square meter"}], "typeOfFlow": "Product flow", "classification": {"classHierarchy": "Gebäudetechnik / Sanitär / Dusch- und Badewannen", "name": "OEKOBAU.DAT"}}, {"dataSetInternalID": 1, "referenceToFlowDataSet": {"shortDescription": [{"value": "Erneuerbare Primärenergie als Energieträger (PERE)", "lang": "de"}, {"value": "Renewable primary energy as energy carrier (PERE)", "lang": "en"}], "type": "flow data set", "refObjectId": "20f32be5-0398-4288-9b6d-accddd195317", "uri": "../flows/20f32be5-0398-4288-9b6d-accddd195317.xml"}, "exchange direction": "INPUT", "other": {"anies": [{"name": "referenceToUnitGroupDataSet", "value": {"shortDescription": [{"value": "MJ", "lang": "de"}], "type": "unit group data set", "refObjectId": "93a60a57-a3c8-11da-a746-0800200c9a66", "uri": "../unitgroups/93a60a57-a3c8-11da-a746-0800200c9a66.xml"}}, {"value": "63.7", "module": "A1"}, {"value": "0", "module": "A2"}, {"value": "1.27", "module": "A3"}, {"value": "0", "module": "C1"}, {"value": "0", "module": "C2"}, {"value": "0", "module": "C3"}, {"value": "0.759", "module": "C4"}, {"value": "-0.0185", "module": "D"}]}, "resolvedFlowVersion": "38.00.000", "flowProperties": [], "typeOfFlow": "Other flow", "classification": {"classHierarchy": "Quantities", "name": "GaBiCategories"}}, {"dataSetInternalID": 2, "referenceToFlowDataSet": {"shortDescription": [{"value": "Erneuerbare Primärenergie zur stofflichen Nutzung (PERM)", "lang": "de"}, {"value": "Renewable primary energy resources as material utilization (PERM)", "lang": "en"}], "type": "flow data set", "refObjectId": "fb3ec0de-548d-4508-aea5-00b73bf6f702", "uri": "../flows/fb3ec0de-548d-4508-aea5-00b73bf6f702.xml"}, "exchange direction": "INPUT", "other": {"anies": [{"name": "referenceToUnitGroupDataSet", "value": {"shortDescription": [{"value": "MJ", "lang": "de"}], "type": "unit group data set", "refObjectId": "93a60a57-a3c8-11da-a746-0800200c9a66", "uri": "../unitgroups/93a60a57-a3c8-11da-a746-0800200c9a66.xml"}}, {"value": "30.6", "module": "A1"}, {"value": "0", "module": "A2"}, {"value": "0.648", "module": "A3"}, {"value": "0", "module": "C1"}, {"value": "0", "module": "C2"}, {"value": "0", "module": "C3"}, {"value": "0.109", "module": "C4"}, {"value": "-0.00238", "module": "D"}]}, "resolvedFlowVersion": "38.00.000", "flowProperties": [], "typeOfFlow": "Other flow", "classification": {"classHierarchy": "Quantities", "name": "GaBiCategories"}}, {"dataSetInternalID": 3, "referenceToFlowDataSet": {"shortDescription": [{"value": "Total erneuerbare Primärenergie (PERT)", "lang": "de"}, {"value": "Total use of renewable primary energy resources (PERT)", "lang": "en"}], "type": "flow data set", "refObjectId": "53f97275-fa8a-4cdd-9024-65936002acd0", "uri": "../flows/53f97275-fa8a-4cdd-9024-65936002acd0.xml"}, "exchange direction": "INPUT", "other": {"anies": [{"name": "referenceToUnitGroupDataSet", "value": {"shortDescription": [{"value": "MJ", "lang": "de"}], "type": "unit group data set", "refObjectId": "93a60a57-a3c8-11da-a746-0800200c9a66", "uri": "../unitgroups/93a60a57-a3c8-11da-a746-0800200c9a66.xml"}}, {"value": "94.2", "module": "A1"}, {"value": "0", "module": "A2"}, {"value": "1.92", "module": "A3"}, {"value": "0", "module": "C1"}, {"value": "0", "module": "C2"}, {"value": "0", "module": "C3"}, {"value": "0.868", "module": "C4"}, {"value": "-0.0209", "module": "D"}]}, "resolvedFlowVersion": "38.00.000", "flowProperties": [], "typeOfFlow": "Other flow", "classification": {"classHierarchy": "Quantities / Environmental quantities / EPD EN 15804 / LCI indicators", "name": "GaBiCategories"}}, {"dataSetInternalID": 4, "referenceToFlowDataSet": {"shortDescription": [{"value": "Nicht-erneuerbare Primärenergie als Energieträger (PENRE)", "lang": "de"}, {"value": "Non renewable primary energy as energy carrier (PENRE)", "lang": "en"}], "type": "flow data set", "refObjectId": "ac857178-2b45-46ec-892a-a9a4332f0372", "uri": "../flows/ac857178-2b45-46ec-892a-a9a4332f0372.xml"}, "exchange direction": "INPUT", "other": {"anies": [{"name": "referenceToUnitGroupDataSet", "value": {"shortDescription": [{"value": "MJ", "lang": "de"}], "type": "unit group data set", "refObjectId": "93a60a57-a3c8-11da-a746-0800200c9a66", "uri": "../unitgroups/93a60a57-a3c8-11da-a746-0800200c9a66.xml"}}, {"value": "320", "module": "A1"}, {"value": "0", "module": "A2"}, {"value": "0", "module": "A3"}, {"value": "0", "module": "C1"}, {"value": "0", "module": "C2"}, {"value": "0", "module": "C3"}, {"value": "0", "module": "C4"}, {"value": "0", "module": "D"}]}, "resolvedFlowVersion": "38.00.000", "flowProperties": [], "typeOfFlow": "Other flow", "classification": {"classHierarchy": "Quantities", "name": "GaBiCategories"}}, {"dataSetInternalID": 5, "referenceToFlowDataSet": {"shortDescription": [{"value": "Nicht-erneuerbare Primärenergie zur stofflichen Nutzung (PENRM)", "lang": "de"}, {"value": "Non renewable primary energy as material utilization (PENRM)", "lang": "en"}], "type": "flow data set", "refObjectId": "1421caa0-679d-4bf4-b282-0eb850ccae27", "uri": "../flows/1421caa0-679d-4bf4-b282-0eb850ccae27.xml"}, "exchange direction": "INPUT", "other": {"anies": [{"name": "referenceToUnitGroupDataSet", "value": {"shortDescription": [{"value": "MJ", "lang": "de"}], "type": "unit group data set", "refObjectId": "93a60a57-a3c8-11da-a746-0800200c9a66", "uri": "../unitgroups/93a60a57-a3c8-11da-a746-0800200c9a66.xml"}}, {"value": "887", "module": "A1"}, {"value": "0", "module": "A2"}, {"value": "11.7", "module": "A3"}, {"value": "0", "module": "C1"}, {"value": "0", "module": "C2"}, {"value": "0", "module": "C3"}, {"value": "8.87", "module": "C4"}, {"value": "-0.286", "module": "D"}]}, "resolvedFlowVersion": "38.00.000", "flowProperties": [], "typeOfFlow": "Other flow", "classification": {"classHierarchy": "Quantities", "name": "GaBiCategories"}}, {"dataSetInternalID": 6, "referenceToFlowDataSet": {"shortDescription": [{"value": "Total nicht erneuerbare Primärenergie (PENRT)", "lang": "de"}, {"value": "Total use of non renewable primary energy resources (PENRT)", "lang": "en"}], "type": "flow data set", "refObjectId": "06159210-646b-4c8d-8583-da9b3b95a6c1", "uri": "../flows/06159210-646b-4c8d-8583-da9b3b95a6c1.xml"}, "exchange direction": "INPUT", "other": {"anies": [{"name": "referenceToUnitGroupDataSet", "value": {"shortDescription": [{"value": "MJ", "lang": "de"}], "type": "unit group data set", "refObjectId": "93a60a57-a3c8-11da-a746-0800200c9a66", "uri": "../unitgroups/93a60a57-a3c8-11da-a746-0800200c9a66.xml"}}, {"value": "1210", "module": "A1"}, {"value": "0", "module": "A2"}, {"value": "11.7", "module": "A3"}, {"value": "0", "module": "C1"}, {"value": "0", "module": "C2"}, {"value": "0", "module": "C3"}, {"value": "8.87", "module": "C4"}, {"value": "-0.286", "module": "D"}]}, "resolvedFlowVersion": "38.00.000", "flowProperties": [], "typeOfFlow": "Other flow", "classification": {"classHierarchy": "Quantities / Environmental quantities / EPD EN 15804 / LCI indicators", "name": "GaBiCategories"}}, {"dataSetInternalID": 7, "referenceToFlowDataSet": {"shortDescription": [{"value": "Einsatz von Sekundärstoffen (SM)", "lang": "de"}, {"value": "Use of secondary material (SM)", "lang": "en"}], "type": "flow data set", "refObjectId": "c6a1f35f-2d09-4f54-8dfb-97e502e1ce92", "uri": "../flows/c6a1f35f-2d09-4f54-8dfb-97e502e1ce92.xml"}, "exchange direction": "INPUT", "other": {"anies": [{"name": "referenceToUnitGroupDataSet", "value": {"shortDescription": [{"value": "kg", "lang": "de"}], "type": "unit group data set", "refObjectId": "ad38d542-3fe9-439d-9b95-2f5f7752acaf", "uri": "../unitgroups/ad38d542-3fe9-439d-9b95-2f5f7752acaf.xml"}}, {"value": "0", "module": "A1"}, {"value": "0", "module": "A2"}, {"value": "0", "module": "A3"}, {"value": "0", "module": "C1"}, {"value": "0", "module": "C2"}, {"value": "0", "module": "C3"}, {"value": "0", "module": "C4"}, {"value": "0", "module": "D"}]}, "resolvedFlowVersion": "38.00.000", "flowProperties": [], "typeOfFlow": "Other flow", "classification": {"classHierarchy": "Quantities / Environmental quantities / EPD EN 15804 / LCI indicators", "name": "GaBiCategories"}}, {"dataSetInternalID": 8, "referenceToFlowDataSet": {"shortDescription": [{"value": "Erneuerbare Sekundärbrennstoffe (RSF)", "lang": "de"}, {"value": "Use of renewable secondary fuels (RSF)", "lang": "en"}], "type": "flow data set", "refObjectId": "64333088-a55f-4aa2-9a31-c10b07816787", "uri": "../flows/64333088-a55f-4aa2-9a31-c10b07816787.xml"}, "exchange direction": "INPUT", "other": {"anies": [{"name": "referenceToUnitGroupDataSet", "value": {"shortDescription": [{"value": "MJ", "lang": "de"}], "type": "unit group data set", "refObjectId": "93a60a57-a3c8-11da-a746-0800200c9a66", "uri": "../unitgroups/93a60a57-a3c8-11da-a746-0800200c9a66.xml"}}, {"value": "0", "module": "A1"}, {"value": "0", "module": "A2"}, {"value": "0", "module": "A3"}, {"value": "0", "module": "C1"}, {"value": "0", "module": "C2"}, {"value": "0", "module": "C3"}, {"value": "0", "module": "C4"}, {"value": "0", "module": "D"}]}, "resolvedFlowVersion": "38.00.000", "flowProperties": [], "typeOfFlow": "Other flow", "classification": {"classHierarchy": "Quantities / Environmental quantities / EPD EN 15804 / LCI indicators", "name": "GaBiCategories"}}, {"dataSetInternalID": 9, "referenceToFlowDataSet": {"shortDescription": [{"value": "Nicht erneuerbare Sekundärbrennstoffe (NRSF)", "lang": "de"}, {"value": "Use of non renewable secondary fuels (NRSF)", "lang": "en"}], "type": "flow data set", "refObjectId": "89def144-d39a-4287-b86f-efde453ddcb2", "uri": "../flows/89def144-d39a-4287-b86f-efde453ddcb2.xml"}, "exchange direction": "INPUT", "other": {"anies": [{"name": "referenceToUnitGroupDataSet", "value": {"shortDescription": [{"value": "MJ", "lang": "de"}], "type": "unit group data set", "refObjectId": "93a60a57-a3c8-11da-a746-0800200c9a66", "uri": "../unitgroups/93a60a57-a3c8-11da-a746-0800200c9a66.xml"}}, {"value": "0", "module": "A1"}, {"value": "0", "module": "A2"}, {"value": "0", "module": "A3"}, {"value": "0", "module": "C1"}, {"value": "0", "module": "C2"}, {"value": "0", "module": "C3"}, {"value": "0", "module": "C4"}, {"value": "0", "module": "D"}]}, "resolvedFlowVersion": "38.00.000", "flowProperties": [], "typeOfFlow": "Other flow", "classification": {"classHierarchy": "Quantities / Environmental quantities / EPD EN 15804 / LCI indicators", "name": "GaBiCategories"}}, {"dataSetInternalID": 10, "referenceToFlowDataSet": {"shortDescription": [{"value": "Einsatz von Süßwasserressourcen (FW)", "lang": "de"}, {"value": "Use of net fresh water (FW)", "lang": "en"}], "type": "flow data set", "refObjectId": "3cf952c8-f3a4-461d-8c96-96456ca62246", "uri": "../flows/3cf952c8-f3a4-461d-8c96-96456ca62246.xml"}, "exchange direction": "INPUT", "other": {"anies": [{"name": "referenceToUnitGroupDataSet", "value": {"shortDescription": [{"value": "m^3", "lang": "de"}], "type": "unit group data set", "refObjectId": "cd950537-0a98-4044-9ba7-9f9a68d0a504", "uri": "../unitgroups/cd950537-0a98-4044-9ba7-9f9a68d0a504.xml"}}, {"value": "0.532", "module": "A1"}, {"value": "0.00228", "module": "A2"}, {"value": "0.00712", "module": "A3"}, {"value": "0", "module": "C1"}, {"value": "0.0011", "module": "C2"}, {"value": "0", "module": "C3"}, {"value": "0.0344", "module": "C4"}, {"value": "-9.99E-05", "module": "D"}]}, "resolvedFlowVersion": "38.00.000", "flowProperties": [], "typeOfFlow": "Other flow", "classification": {"classHierarchy": "Quantities / Environmental quantities / EPD EN 15804 / LCI indicators", "name": "GaBiCategories"}}, {"dataSetInternalID": 11, "referenceToFlowDataSet": {"shortDescription": [{"value": "Gefährlicher Abfall zur Deponie (HWD)", "lang": "de"}, {"value": "Hazardous waste disposed (HWD)", "lang": "en"}], "type": "flow data set", "refObjectId": "430f9e0f-59b2-46a0-8e0d-55e0e84948fc", "uri": "../flows/430f9e0f-59b2-46a0-8e0d-55e0e84948fc.xml"}, "exchange direction": "OUTPUT", "other": {"anies": [{"name": "referenceToUnitGroupDataSet", "value": {"shortDescription": [{"value": "kg", "lang": "de"}], "type": "unit group data set", "refObjectId": "ad38d542-3fe9-439d-9b95-2f5f7752acaf", "uri": "../unitgroups/ad38d542-3fe9-439d-9b95-2f5f7752acaf.xml"}}, {"value": "0.00042", "module": "A1"}, {"value": "4.79E-05", "module": "A2"}, {"value": "7.44E-05", "module": "A3"}, {"value": "0", "module": "C1"}, {"value": "8.38E-05", "module": "C2"}, {"value": "0", "module": "C3"}, {"value": "1.48E-05", "module": "C4"}, {"value": "-2.24E-07", "module": "D"}]}, "resolvedFlowVersion": "38.00.000", "flowProperties": [], "typeOfFlow": "Other flow", "classification": {"classHierarchy": "Quantities / Environmental quantities / EPD EN 15804 / LCI indicators", "name": "GaBiCategories"}}, {"dataSetInternalID": 12, "referenceToFlowDataSet": {"shortDescription": [{"value": "Entsorgter nicht gefährlicher Abfall (NHWD)", "lang": "de"}, {"value": "Non hazardous waste disposed (NHWD)", "lang": "en"}], "type": "flow data set", "refObjectId": "b29ef66b-e286-4afa-949f-62f1a7b4d7fa", "uri": "../flows/b29ef66b-e286-4afa-949f-62f1a7b4d7fa.xml"}, "exchange direction": "OUTPUT", "other": {"anies": [{"name": "referenceToUnitGroupDataSet", "value": {"shortDescription": [{"value": "kg", "lang": "de"}], "type": "unit group data set", "refObjectId": "ad38d542-3fe9-439d-9b95-2f5f7752acaf", "uri": "../unitgroups/ad38d542-3fe9-439d-9b95-2f5f7752acaf.xml"}}, {"value": "2.67", "module": "A1"}, {"value": "0.991", "module": "A2"}, {"value": "0.405", "module": "A3"}, {"value": "0", "module": "C1"}, {"value": "0.148", "module": "C2"}, {"value": "0", "module": "C3"}, {"value": "0.601", "module": "C4"}, {"value": "0", "module": "D"}]}, "resolvedFlowVersion": "38.00.000", "flowProperties": [], "typeOfFlow": "Other flow", "classification": {"classHierarchy": "Quantities / Environmental quantities / EPD EN 15804 / LCI indicators", "name": "GaBiCategories"}}, {"dataSetInternalID": 13, "referenceToFlowDataSet": {"shortDescription": [{"value": "Entsorgter radioaktiver Abfall (RWD)", "lang": "de"}, {"value": "Radioactive waste disposed (RWD)", "lang": "en"}], "type": "flow data set", "refObjectId": "3449546e-52ad-4b39-b809-9fb77cea8ff6", "uri": "../flows/3449546e-52ad-4b39-b809-9fb77cea8ff6.xml"}, "exchange direction": "OUTPUT", "other": {"anies": [{"name": "referenceToUnitGroupDataSet", "value": {"shortDescription": [{"value": "kg", "lang": "de"}], "type": "unit group data set", "refObjectId": "ad38d542-3fe9-439d-9b95-2f5f7752acaf", "uri": "../unitgroups/ad38d542-3fe9-439d-9b95-2f5f7752acaf.xml"}}, {"value": "0", "module": "A1"}, {"value": "0.000158", "module": "A2"}, {"value": "3.29E-05", "module": "A3"}, {"value": "0", "module": "C1"}, {"value": "0.000221", "module": "C2"}, {"value": "0", "module": "C3"}, {"value": "2.57E-05", "module": "C4"}, {"value": "-5.52E-07", "module": "D"}]}, "resolvedFlowVersion": "38.00.000", "flowProperties": [], "typeOfFlow": "Other flow", "classification": {"classHierarchy": "Quantities / Environmental quantities / EPD EN 15804 / LCI indicators", "name": "GaBiCategories"}}, {"dataSetInternalID": 14, "referenceToFlowDataSet": {"shortDescription": [{"value": "Komponenten für die Wiederverwendung (CRU)", "lang": "de"}, {"value": "Components for re-use (CRU)", "lang": "en"}], "type": "flow data set", "refObjectId": "a2b32f97-3fc7-4af2-b209-525bc6426f33", "uri": "../flows/a2b32f97-3fc7-4af2-b209-525bc6426f33.xml"}, "exchange direction": "OUTPUT", "other": {"anies": [{"name": "referenceToUnitGroupDataSet", "value": {"shortDescription": [{"value": "kg", "lang": "de"}], "type": "unit group data set", "refObjectId": "ad38d542-3fe9-439d-9b95-2f5f7752acaf", "uri": "../unitgroups/ad38d542-3fe9-439d-9b95-2f5f7752acaf.xml"}}, {"value": "0", "module": "A1"}, {"value": "0", "module": "A2"}, {"value": "0", "module": "A3"}, {"value": "0", "module": "C1"}, {"value": "0", "module": "C2"}, {"value": "0", "module": "C3"}, {"value": "0", "module": "C4"}, {"value": "0", "module": "D"}]}, "resolvedFlowVersion": "38.00.000", "flowProperties": [], "typeOfFlow": "Other flow", "classification": {"classHierarchy": "Quantities / Environmental quantities / EPD EN 15804 / LCI indicators", "name": "GaBiCategories"}}, {"dataSetInternalID": 15, "referenceToFlowDataSet": {"shortDescription": [{"value": "Stoffe zum Recycling (MFR)", "lang": "de"}, {"value": "Materials for recycling (MFR)", "lang": "en"}], "type": "flow data set", "refObjectId": "d7fe48a5-4103-49c8-9aae-b0b5dfdbd6ae", "uri": "../flows/d7fe48a5-4103-49c8-9aae-b0b5dfdbd6ae.xml"}, "exchange direction": "OUTPUT", "other": {"anies": [{"name": "referenceToUnitGroupDataSet", "value": {"shortDescription": [{"value": "kg", "lang": "de"}], "type": "unit group data set", "refObjectId": "ad38d542-3fe9-439d-9b95-2f5f7752acaf", "uri": "../unitgroups/ad38d542-3fe9-439d-9b95-2f5f7752acaf.xml"}}, {"value": "0", "module": "A1"}, {"value": "0", "module": "A2"}, {"value": "0.254", "module": "A3"}, {"value": "0", "module": "C1"}, {"value": "0", "module": "C2"}, {"value": "0", "module": "C3"}, {"value": "0.254", "module": "C4"}, {"value": "0", "module": "D"}]}, "resolvedFlowVersion": "38.00.000", "flowProperties": [], "typeOfFlow": "Other flow", "classification": {"classHierarchy": "Quantities / Environmental quantities / EPD EN 15804 / LCI indicators", "name": "GaBiCategories"}}, {"dataSetInternalID": 16, "referenceToFlowDataSet": {"shortDescription": [{"value": "Stoffe für die Energierückgewinnung (MER)", "lang": "de"}, {"value": "Materials for energy recovery (MER)", "lang": "en"}], "type": "flow data set", "refObjectId": "59a9181c-3aaf-46ee-8b13-2b3723b6e447", "uri": "../flows/59a9181c-3aaf-46ee-8b13-2b3723b6e447.xml"}, "exchange direction": "OUTPUT", "other": {"anies": [{"name": "referenceToUnitGroupDataSet", "value": {"shortDescription": [{"value": "kg", "lang": "de"}], "type": "unit group data set", "refObjectId": "ad38d542-3fe9-439d-9b95-2f5f7752acaf", "uri": "../unitgroups/ad38d542-3fe9-439d-9b95-2f5f7752acaf.xml"}}, {"value": "0", "module": "A1"}, {"value": "0", "module": "A2"}, {"value": "0", "module": "A3"}, {"value": "0", "module": "C1"}, {"value": "0", "module": "C2"}, {"value": "0", "module": "C3"}, {"value": "0", "module": "C4"}, {"value": "0", "module": "D"}]}, "resolvedFlowVersion": "38.00.000", "flowProperties": [], "typeOfFlow": "Other flow", "classification": {"classHierarchy": "Quantities / Environmental quantities / EPD EN 15804 / LCI indicators", "name": "GaBiCategories"}}, {"dataSetInternalID": 17, "referenceToFlowDataSet": {"shortDescription": [{"value": "Exportierte elektrische Energie (EEE)", "lang": "de"}, {"value": "Exported electrical energy (EEE)", "lang": "en"}], "type": "flow data set", "refObjectId": "4da0c987-2b76-40d6-9e9e-82a017aaaf29", "uri": "../flows/4da0c987-2b76-40d6-9e9e-82a017aaaf29.xml"}, "exchange direction": "OUTPUT", "other": {"anies": [{"name": "referenceToUnitGroupDataSet", "value": {"shortDescription": [{"value": "MJ", "lang": "de"}], "type": "unit group data set", "refObjectId": "93a60a57-a3c8-11da-a746-0800200c9a66", "uri": "../unitgroups/93a60a57-a3c8-11da-a746-0800200c9a66.xml"}}, {"value": "0", "module": "A1"}, {"value": "0", "module": "A2"}, {"value": "0", "module": "A3"}, {"value": "0", "module": "C1"}, {"value": "0", "module": "C2"}, {"value": "0", "module": "C3"}, {"value": "9.74", "module": "C4"}, {"value": "0", "module": "D"}]}, "resolvedFlowVersion": "38.00.000", "flowProperties": [], "typeOfFlow": "Other flow", "classification": {"classHierarchy": "Quantities / Environmental quantities / EPD EN 15804 / LCI indicators", "name": "GaBiCategories"}}, {"dataSetInternalID": 18, "referenceToFlowDataSet": {"shortDescription": [{"value": "Exportierte thermische Energie (EET)", "lang": "de"}, {"value": "Exported thermal energy (EET)", "lang": "en"}], "type": "flow data set", "refObjectId": "98daf38a-7a79-46d3-9a37-2b7bd0955810", "uri": "../flows/98daf38a-7a79-46d3-9a37-2b7bd0955810.xml"}, "exchange direction": "OUTPUT", "other": {"anies": [{"name": "referenceToUnitGroupDataSet", "value": {"shortDescription": [{"value": "MJ", "lang": "de"}], "type": "unit group data set", "refObjectId": "93a60a57-a3c8-11da-a746-0800200c9a66", "uri": "../unitgroups/93a60a57-a3c8-11da-a746-0800200c9a66.xml"}}, {"value": "0", "module": "A1"}, {"value": "0", "module": "A2"}, {"value": "0", "module": "A3"}, {"value": "0", "module": "C1"}, {"value": "0", "module": "C2"}, {"value": "0", "module": "C3"}, {"value": "0", "module": "C4"}, {"value": "0", "module": "D"}]}, "resolvedFlowVersion": "38.00.000", "flowProperties": [], "typeOfFlow": "Other flow", "classification": {"classHierarchy": "Quantities / Environmental quantities / EPD EN 15804 / LCI indicators", "name": "GaBiCategories"}}]}, "LCIAResults": {"LCIAResult": [{"referenceToLCIAMethodDataSet": {"shortDescription": [{"value": "Globales Erwärmungspotenzial total (GWP-total)", "lang": "de"}, {"value": "Global Warming Potential total (GWP-total)", "lang": "en"}], "type": "LCIA method data set", "refObjectId": "6a37f984-a4b3-458a-a20a-64418c145fa2", "uri": "../lciamethods/6a37f984-a4b3-458a-a20a-64418c145fa2.xml"}, "other": {"anies": [{"name": "referenceToUnitGroupDataSet", "value": {"shortDescription": [{"value": "kg CO_(2)-Äq.", "lang": "de"}], "type": "unit group data set", "refObjectId": "1ebf3012-d0db-4de2-aefd-ef30cedb0be1", "uri": "../unitgroups/1ebf3012-d0db-4de2-aefd-ef30cedb0be1.xml"}}, {"value": "71.9", "module": "A1"}, {"value": "1.67", "module": "A2"}, {"value": "4.17", "module": "A3"}, {"value": "0", "module": "C1"}, {"value": "2.29", "module": "C2"}, {"value": "0", "module": "C3"}, {"value": "27.2", "module": "C4"}, {"value": "-0.0207", "module": "D"}]}}, {"referenceToLCIAMethodDataSet": {"shortDescription": [{"value": "Globales Erwärmungspotenzial fossil (GWP-fossil)", "lang": "de"}, {"value": "Global Warming Potential fossil fuels (GWP-fossil)", "lang": "en"}], "type": "LCIA method data set", "refObjectId": "5f635281-343e-44fb-83df-1971b155e6b6", "uri": "../lciamethods/5f635281-343e-44fb-83df-1971b155e6b6.xml"}, "other": {"anies": [{"name": "referenceToUnitGroupDataSet", "value": {"shortDescription": [{"value": "kg CO_(2)-Äq.", "lang": "de"}], "type": "unit group data set", "refObjectId": "1ebf3012-d0db-4de2-aefd-ef30cedb0be1", "uri": "../unitgroups/1ebf3012-d0db-4de2-aefd-ef30cedb0be1.xml"}}, {"value": "78.9", "module": "A1"}, {"value": "1.66", "module": "A2"}, {"value": "4.51", "module": "A3"}, {"value": "0", "module": "C1"}, {"value": "2.29", "module": "C2"}, {"value": "0", "module": "C3"}, {"value": "20.2", "module": "C4"}, {"value": "-0.0206", "module": "D"}]}}, {"referenceToLCIAMethodDataSet": {"shortDescription": [{"value": "Globales Erwärmungspotenzial biogen (GWP-biogenic)", "lang": "de"}, {"value": "Global Warming Potential biogenic (GWP-biogenic)", "lang": "en"}], "type": "LCIA method data set", "refObjectId": "2356e1ab-0185-4db5-86e5-16de51c7485c", "uri": "../lciamethods/2356e1ab-0185-4db5-86e5-16de51c7485c.xml"}, "other": {"anies": [{"name": "referenceToUnitGroupDataSet", "value": {"shortDescription": [{"value": "kg CO_(2)-Äq.", "lang": "de"}], "type": "unit group data set", "refObjectId": "1ebf3012-d0db-4de2-aefd-ef30cedb0be1", "uri": "../unitgroups/1ebf3012-d0db-4de2-aefd-ef30cedb0be1.xml"}}, {"value": "-6.99", "module": "A1"}, {"value": "0.000288", "module": "A2"}, {"value": "-0.339", "module": "A3"}, {"value": "0", "module": "C1"}, {"value": "0.000625", "module": "C2"}, {"value": "0", "module": "C3"}, {"value": "6.99", "module": "C4"}, {"value": "-5.77E-05", "module": "D"}]}}, {"referenceToLCIAMethodDataSet": {"shortDescription": [{"value": "Globales Erwärmungspotenzial luluc (GWP-luluc)", "lang": "de"}, {"value": "Global Warming Potential luluc (GWP-luluc)", "lang": "en"}], "type": "LCIA method data set", "refObjectId": "4331bbdb-978a-490d-8707-eeb047f01a55", "uri": "../lciamethods/4331bbdb-978a-490d-8707-eeb047f01a55.xml"}, "other": {"anies": [{"name": "referenceToUnitGroupDataSet", "value": {"shortDescription": [{"value": "kg CO_(2)-Äq.", "lang": "de"}], "type": "unit group data set", "refObjectId": "1ebf3012-d0db-4de2-aefd-ef30cedb0be1", "uri": "../unitgroups/1ebf3012-d0db-4de2-aefd-ef30cedb0be1.xml"}}, {"value": "0.0152", "module": "A1"}, {"value": "0.000804", "module": "A2"}, {"value": "0.00141", "module": "A3"}, {"value": "0", "module": "C1"}, {"value": "0.000212", "module": "C2"}, {"value": "0", "module": "C3"}, {"value": "0.000918", "module": "C4"}, {"value": "-2.35E-05", "module": "D"}]}}, {"referenceToLCIAMethodDataSet": {"shortDescription": [{"value": "Abbau Potential der stratosphärischen Ozonschicht (ODP)", "lang": "de"}, {"value": "Depletion potential of the stratospheric ozone layer (ODP)", "lang": "en"}], "type": "LCIA method data set", "refObjectId": "b5c629d6-def3-11e6-bf01-fe55135034f3", "uri": "../lciamethods/b5c629d6-def3-11e6-bf01-fe55135034f3.xml"}, "other": {"anies": [{"name": "referenceToUnitGroupDataSet", "value": {"shortDescription": [{"value": "kg CFC11-Äq.", "lang": "de"}], "type": "unit group data set", "refObjectId": "d9e957c9-7309-4474-bf3a-7777df6c4e5b", "uri": "../unitgroups/d9e957c9-7309-4474-bf3a-7777df6c4e5b.xml"}}, {"value": "3.6E-06", "module": "A1"}, {"value": "3.55E-07", "module": "A2"}, {"value": "8.96E-08", "module": "A3"}, {"value": "0", "module": "C1"}, {"value": "4.99E-07", "module": "C2"}, {"value": "0", "module": "C3"}, {"value": "6.68E-08", "module": "C4"}, {"value": "-1.48E-09", "module": "D"}]}}, {"referenceToLCIAMethodDataSet": {"shortDescription": [{"value": "Versauerungspotenzial von Boden und Wasser (AP)", "lang": "de"}, {"value": "Acidification potential of land and water (AP)", "lang": "en"}], "type": "LCIA method data set", "refObjectId": "b5c611c6-def3-11e6-bf01-fe55135034f3", "uri": "../lciamethods/b5c611c6-def3-11e6-bf01-fe55135034f3.xml"}, "other": {"anies": [{"name": "referenceToUnitGroupDataSet", "value": {"shortDescription": [{"value": "mol H^(+)-Äq.", "lang": "de"}], "type": "unit group data set", "refObjectId": "42e089ac-92bf-4bf2-8ca1-5fc40d18f2ed", "uri": "../unitgroups/42e089ac-92bf-4bf2-8ca1-5fc40d18f2ed.xml"}}, {"value": "0.394", "module": "A1"}, {"value": "0.0258", "module": "A2"}, {"value": "0.00519", "module": "A3"}, {"value": "0", "module": "C1"}, {"value": "0.0145", "module": "C2"}, {"value": "0", "module": "C3"}, {"value": "0.0069", "module": "C4"}, {"value": "-7.45E-05", "module": "D"}]}}, {"referenceToLCIAMethodDataSet": {"shortDescription": [{"value": "Eutrophierungspotenzial Süßwasser (EP-freshwater)", "lang": "de"}, {"value": "Eutrophication potential aquatic freshwater (EP-freshwater)", "lang": "en"}], "type": "LCIA method data set", "refObjectId": "b53ec18f-7377-4ad3-86eb-cc3f4f276b2b", "uri": "../lciamethods/b53ec18f-7377-4ad3-86eb-cc3f4f276b2b.xml"}, "other": {"anies": [{"name": "referenceToUnitGroupDataSet", "value": {"shortDescription": [{"value": "kg PO_(4)-Äq.", "lang": "de"}], "type": "unit group data set", "refObjectId": "0429039d-a61d-4590-ba67-aa4a20a810a1", "uri": "../unitgroups/0429039d-a61d-4590-ba67-aa4a20a810a1.xml"}}, {"value": "0.00774", "module": "A1"}, {"value": "0.000116", "module": "A2"}, {"value": "0.000282", "module": "A3"}, {"value": "0", "module": "C1"}, {"value": "4.79E-05", "module": "C2"}, {"value": "0", "module": "C3"}, {"value": "0.000256", "module": "C4"}, {"value": "-6.44E-06", "module": "D"}]}}, {"referenceToLCIAMethodDataSet": {"shortDescription": [{"value": "Eutrophierungspotenzial Salzwasser (EP-marine)", "lang": "de"}, {"value": "Eutrophication potential aquatic marine (EP-marine)", "lang": "en"}], "type": "LCIA method data set", "refObjectId": "b5c619fa-def3-11e6-bf01-fe55135034f3", "uri": "../lciamethods/b5c619fa-def3-11e6-bf01-fe55135034f3.xml"}, "other": {"anies": [{"name": "referenceToUnitGroupDataSet", "value": {"shortDescription": [{"value": "kg N-Äq.", "lang": "de"}], "type": "unit group data set", "refObjectId": "d05bb823-ecdf-4686-8c40-bf1d9257859f", "uri": "../unitgroups/d05bb823-ecdf-4686-8c40-bf1d9257859f.xml"}}, {"value": "0.0644", "module": "A1"}, {"value": "0.00699", "module": "A2"}, {"value": "0.00249", "module": "A3"}, {"value": "0", "module": "C1"}, {"value": "0.00582", "module": "C2"}, {"value": "0", "module": "C3"}, {"value": "0.00313", "module": "C4"}, {"value": "-1.47E-05", "module": "D"}]}}, {"referenceToLCIAMethodDataSet": {"shortDescription": [{"value": "Eutrophierungspotenzial Land (EP-terrestrial)", "lang": "de"}, {"value": "Eutrophication potential terrestrial (EP-terrestrial)", "lang": "en"}], "type": "LCIA method data set", "refObjectId": "b5c614d2-def3-11e6-bf01-fe55135034f3", "uri": "../lciamethods/b5c614d2-def3-11e6-bf01-fe55135034f3.xml"}, "other": {"anies": [{"name": "referenceToUnitGroupDataSet", "value": {"shortDescription": [{"value": "mol N-Äq.", "lang": "de"}], "type": "unit group data set", "refObjectId": "71b4d617-0ec9-4d3f-b65e-e438940c2401", "uri": "../unitgroups/71b4d617-0ec9-4d3f-b65e-e438940c2401.xml"}}, {"value": "0.62", "module": "A1"}, {"value": "0.0773", "module": "A2"}, {"value": "0.0159", "module": "A3"}, {"value": "0", "module": "C1"}, {"value": "0.0639", "module": "C2"}, {"value": "0", "module": "C3"}, {"value": "0.0273", "module": "C4"}, {"value": "-0.00015", "module": "D"}]}}, {"referenceToLCIAMethodDataSet": {"shortDescription": [{"value": "Bildungspotential für troposphärisches Ozon (POCP)", "lang": "de"}, {"value": "Formation potential of tropospheric ozone photochemical oxidants (POCP)", "lang": "en"}], "type": "LCIA method data set", "refObjectId": "b5c610fe-def3-11e6-bf01-fe55135034f3", "uri": "../lciamethods/b5c610fe-def3-11e6-bf01-fe55135034f3.xml"}, "other": {"anies": [{"name": "referenceToUnitGroupDataSet", "value": {"shortDescription": [{"value": "kg NMVOC-Äq.", "lang": "de"}], "type": "unit group data set", "refObjectId": "d27c25f8-fbc1-44c6-b47b-4adbae4199c6", "uri": "../unitgroups/d27c25f8-fbc1-44c6-b47b-4adbae4199c6.xml"}}, {"value": "0.269", "module": "A1"}, {"value": "0.0206", "module": "A2"}, {"value": "0.134", "module": "A3"}, {"value": "0", "module": "C1"}, {"value": "0.0225", "module": "C2"}, {"value": "0", "module": "C3"}, {"value": "0.00671", "module": "C4"}, {"value": "-4.28E-05", "module": "D"}]}}, {"referenceToLCIAMethodDataSet": {"shortDescription": [{"value": "Potenzial für den abiotischen Abbau nicht fossiler Ressourcen (ADPE)", "lang": "de"}, {"value": "Abiotic depletion potential for non fossil resources (ADPE)", "lang": "en"}], "type": "LCIA method data set", "refObjectId": "b2ad6494-c78d-11e6-9d9d-cec0c932ce01", "uri": "../lciamethods/b2ad6494-c78d-11e6-9d9d-cec0c932ce01.xml"}, "other": {"anies": [{"name": "referenceToUnitGroupDataSet", "value": {"shortDescription": [{"value": "kg Sb-Äq.", "lang": "de"}], "type": "unit group data set", "refObjectId": "54ccd2d9-a32a-4fc2-923d-f2c8c93e89d4", "uri": "../unitgroups/54ccd2d9-a32a-4fc2-923d-f2c8c93e89d4.xml"}}, {"value": "0.000611", "module": "A1"}, {"value": "3.11E-05", "module": "A2"}, {"value": "7.74E-05", "module": "A3"}, {"value": "0", "module": "C1"}, {"value": "1.35E-05", "module": "C2"}, {"value": "0", "module": "C3"}, {"value": "8.5E-06", "module": "C4"}, {"value": "-2.56E-08", "module": "D"}]}}, {"referenceToLCIAMethodDataSet": {"shortDescription": [{"value": "Potenzial für den abiotischen Abbau fossiler Brennstoffe (ADPF)", "lang": "de"}, {"value": "Abiotic depletion potential for fossil resources (ADPF)", "lang": "en"}], "type": "LCIA method data set", "refObjectId": "b2ad6110-c78d-11e6-9d9d-cec0c932ce01", "uri": "../lciamethods/b2ad6110-c78d-11e6-9d9d-cec0c932ce01.xml"}, "other": {"anies": [{"name": "referenceToUnitGroupDataSet", "value": {"shortDescription": [{"value": "MJ", "lang": "de"}], "type": "unit group data set", "refObjectId": "93a60a57-a3c8-11da-a746-0800200c9a66", "uri": "../unitgroups/93a60a57-a3c8-11da-a746-0800200c9a66.xml"}}, {"value": "1210", "module": "A1"}, {"value": "23.6", "module": "A2"}, {"value": "11.7", "module": "A3"}, {"value": "0", "module": "C1"}, {"value": "31.2", "module": "C2"}, {"value": "0", "module": "C3"}, {"value": "8.87", "module": "C4"}, {"value": "-0.287", "module": "D"}]}}, {"referenceToLCIAMethodDataSet": {"shortDescription": [{"value": "Wassernutzung (WDP)", "lang": "de"}, {"value": "Water use (WDP)", "lang": "en"}], "type": "LCIA method data set", "refObjectId": "b2ad66ce-c78d-11e6-9d9d-cec0c932ce01", "uri": "../lciamethods/b2ad66ce-c78d-11e6-9d9d-cec0c932ce01.xml"}, "other": {"anies": [{"name": "referenceToUnitGroupDataSet", "value": {"shortDescription": [{"value": "m^(3) Welt-Äq. entzogen", "lang": "de"}], "type": "unit group data set", "refObjectId": "6ae2df01-888e-46c8-b17d-49fa3869b476", "uri": "../unitgroups/6ae2df01-888e-46c8-b17d-49fa3869b476.xml"}}, {"value": "20.9", "module": "A1"}, {"value": "0.0669", "module": "A2"}, {"value": "0.255", "module": "A3"}, {"value": "0", "module": "C1"}, {"value": "0.0248", "module": "C2"}, {"value": "0", "module": "C3"}, {"value": "1.07", "module": "C4"}, {"value": "-0.00222", "module": "D"}]}}, {"referenceToLCIAMethodDataSet": {"shortDescription": [{"value": "Auftreten von Krankheiten aufgrund von Feinstaubemissionen (PM)", "lang": "de"}, {"value": "Incidence of disease due to PM emissions (PM)", "lang": "en"}], "type": "LCIA method data set", "refObjectId": "b5c602c6-def3-11e6-bf01-fe55135034f3", "uri": "../lciamethods/b5c602c6-def3-11e6-bf01-fe55135034f3.xml"}, "other": {"anies": [{"name": "referenceToUnitGroupDataSet", "value": {"shortDescription": [{"value": "Krankheitsfälle", "lang": "de"}], "type": "unit group data set", "refObjectId": "3883559b-648f-4afc-8ba2-0bd24f3affa3", "uri": "../unitgroups/3883559b-648f-4afc-8ba2-0bd24f3affa3.xml"}}, {"value": "3.35E-06", "module": "A1"}, {"value": "1.13E-07", "module": "A2"}, {"value": "3.79E-07", "module": "A3"}, {"value": "0", "module": "C1"}, {"value": "3.1E-07", "module": "C2"}, {"value": "0", "module": "C3"}, {"value": "3.77E-08", "module": "C4"}, {"value": "-4.96E-10", "module": "D"}]}}, {"referenceToLCIAMethodDataSet": {"shortDescription": [{"value": "Wirkung durch Exposition des Menschen mit U235 (IR)", "lang": "de"}, {"value": "Human exposure efficiency relative to U235 (IR)", "lang": "en"}], "type": "LCIA method data set", "refObjectId": "b5c632be-def3-11e6-bf01-fe55135034f3", "uri": "../lciamethods/b5c632be-def3-11e6-bf01-fe55135034f3.xml"}, "other": {"anies": [{"name": "referenceToUnitGroupDataSet", "value": {"shortDescription": [{"value": "kBq U235-Äq.", "lang": "de"}], "type": "unit group data set", "refObjectId": "456b05bf-1415-44a9-9993-02452f554c09", "uri": "../unitgroups/456b05bf-1415-44a9-9993-02452f554c09.xml"}}, {"value": "1.62", "module": "A1"}, {"value": "0.11", "module": "A2"}, {"value": "0.04", "module": "A3"}, {"value": "0", "module": "C1"}, {"value": "0.141", "module": "C2"}, {"value": "0", "module": "C3"}, {"value": "0.0688", "module": "C4"}, {"value": "-0.0019", "module": "D"}]}}, {"referenceToLCIAMethodDataSet": {"shortDescription": [{"value": "Toxizitätsvergleichseinheit für Ökosysteme (ETP-fw)", "lang": "de"}, {"value": "Comparative toxic unit for ecosystems (ETP-fw)", "lang": "en"}], "type": "LCIA method data set", "refObjectId": "ee1082d1-b0f7-43ca-a1f0-21e2a4a74511", "uri": "../lciamethods/ee1082d1-b0f7-43ca-a1f0-21e2a4a74511.xml"}, "other": {"anies": [{"name": "referenceToUnitGroupDataSet", "value": {"shortDescription": [{"value": "CTUe", "lang": "de"}], "type": "unit group data set", "refObjectId": "aa959ded-f1eb-4efb-9c5c-2d60be36b3e6", "uri": "../unitgroups/aa959ded-f1eb-4efb-9c5c-2d60be36b3e6.xml"}}, {"value": "1130", "module": "A1"}, {"value": "19.1", "module": "A2"}, {"value": "863", "module": "A3"}, {"value": "0", "module": "C1"}, {"value": "17.8", "module": "C2"}, {"value": "0", "module": "C3"}, {"value": "51.6", "module": "C4"}, {"value": "-0.251", "module": "D"}]}}, {"referenceToLCIAMethodDataSet": {"shortDescription": [{"value": "Toxizitätsvergleichseinheit für Menschen (krebserregend) (HTP-c)", "lang": "de"}, {"value": "Comparative toxic unit for humans (carcinogenic) (HTP-c)", "lang": "en"}], "type": "LCIA method data set", "refObjectId": "2299222a-bbd8-474f-9d4f-4dd1f18aea7c", "uri": "../lciamethods/2299222a-bbd8-474f-9d4f-4dd1f18aea7c.xml"}, "other": {"anies": [{"name": "referenceToUnitGroupDataSet", "value": {"shortDescription": [{"value": "CTUh", "lang": "de"}], "type": "unit group data set", "refObjectId": "d4c9523e-2d7e-49fd-8469-998f547d3a70", "uri": "../unitgroups/d4c9523e-2d7e-49fd-8469-998f547d3a70.xml"}}, {"value": "2.79E-08", "module": "A1"}, {"value": "8.04E-10", "module": "A2"}, {"value": "7.07E-09", "module": "A3"}, {"value": "0", "module": "C1"}, {"value": "2.87E-10", "module": "C2"}, {"value": "0", "module": "C3"}, {"value": "1.96E-09", "module": "C4"}, {"value": "-3.38E-12", "module": "D"}]}}, {"referenceToLCIAMethodDataSet": {"shortDescription": [{"value": "Toxizitätsvergleichseinheit für Menschen (nicht krebserregend) (HTP-nc)", "lang": "de"}, {"value": "Comparative toxic unit for humans (noncarcinogenic) (HTP-nc)", "lang": "en"}], "type": "LCIA method data set", "refObjectId": "3af763a5-b7a1-48c9-9cee-1f223481fcef", "uri": "../lciamethods/3af763a5-b7a1-48c9-9cee-1f223481fcef.xml"}, "other": {"anies": [{"name": "referenceToUnitGroupDataSet", "value": {"shortDescription": [{"value": "CTUh", "lang": "de"}], "type": "unit group data set", "refObjectId": "d4c9523e-2d7e-49fd-8469-998f547d3a70", "uri": "../unitgroups/d4c9523e-2d7e-49fd-8469-998f547d3a70.xml"}}, {"value": "8.95E-07", "module": "A1"}, {"value": "1.95E-08", "module": "A2"}, {"value": "4.6E-08", "module": "A3"}, {"value": "0", "module": "C1"}, {"value": "1.24E-08", "module": "C2"}, {"value": "0", "module": "C3"}, {"value": "7.68E-08", "module": "C4"}, {"value": "-1.27E-10", "module": "D"}]}}, {"referenceToLCIAMethodDataSet": {"shortDescription": [{"value": "Bodenqualitätsindex (SQP)", "lang": "de"}, {"value": "Soil quality index (SQP)", "lang": "en"}], "type": "LCIA method data set", "refObjectId": "b2ad6890-c78d-11e6-9d9d-cec0c932ce01", "uri": "../lciamethods/b2ad6890-c78d-11e6-9d9d-cec0c932ce01.xml"}, "other": {"anies": [{"name": "referenceToUnitGroupDataSet", "value": {"shortDescription": [{"value": "SQP", "lang": "de"}], "type": "unit group data set", "refObjectId": "f130951c-e67f-4f7f-8dd4-665de3974e18", "uri": "../unitgroups/f130951c-e67f-4f7f-8dd4-665de3974e18.xml"}}, {"value": "323", "module": "A1"}, {"value": "14.4", "module": "A2"}, {"value": "6.6", "module": "A3"}, {"value": "0", "module": "C1"}, {"value": "5.43", "module": "C2"}, {"value": "0", "module": "C3"}, {"value": "2.1", "module": "C4"}, {"value": "-0.0297", "module": "D"}]}}]}, "otherAttributes": {"{http://www.indata.network/EPD/2019}epd-version": "1.2"}, "version": "1.1", "locations": "../ILCDLocations.xml"}