{"processInformation": {"dataSetInformation": {"UUID": "280d02e6-e50c-45ff-8ccf-e5b76cf99b56", "name": {"baseName": [{"value": "RAUPIANO PLUS", "lang": "de"}, {"value": "RAUPIANO PLUS", "lang": "en"}], "functionalUnitFlowProperties": [{"lang": "de"}]}, "classificationInformation": {"classification": [{"class": [{"value": "Kunststoffe", "level": 0, "classId": "6"}, {"value": "Rohre", "level": 1, "classId": "6.1"}, {"value": "Abwasserrohre", "level": 2, "classId": "6.1.02"}], "name": "OEKOBAU.DAT"}, {"class": [{"value": "03 Gebäudetechnik", "level": 0}, {"value": "Anlagen zur Wasserversorgung und -entsorgung", "level": 1}, {"value": "Drucklose Abwasserrohrsysteme aus Kunststoff", "level": 2}], "name": "IBUCategories"}]}, "generalComment": [{"value": "Die vorliegende Studie bezieht sich auf die Herstellung des kompletten Rohrsystems, bestehend aus Rohren und Formteilen mit jeweils eingelegtem Dichtungsring in den verschiedenen Durchmessern der Produktpalette. Bei dem zu deklarierenden Rohrsystem handelt es sich um ein 3-schichtiges Rohrsystem aus PP bzw. Mineralstoff-geflltem PP. \nRAUPIANO PLUS ist ein schalldmmendes Hausabflussrohrsystem und erfllt die Anforderungen der EN 1451-1 gem der allgemeinen bauaufsichtlichen Zulassung. Die Rohrdimensionen von DN 32 bis DN 200 entsprechend der EN 1451-1 gestatten den problemlosen bergang auf konventionelle (nicht-schalldmmende) PP-Rohrsysteme nach EN 1451-1 bzw. auf Kanalrohrsystems nach EN 1401-1.\n\n\nDer 3-schichtige Aufbau von RAUPIANO PLUS fhrt zu einer erhhten Rohrsteifigkeit. Nummer 1 zeigt eine abriebfeste und hochgleitfhige Innenschicht aus PP. Nummer 2 besteht aus einer hochsteifen Mittelschicht aus mineralverstrktem PP und Nummer 3 ist eine schlagzhe und stofeste PP-Auenschicht.", "lang": "de"}, {"value": "This study covers the manufacturing of the complete pipe system consisting of pipes and fittings with fitted sealing ring, in the different dimensions of the product range. The declared pipe system is a three-layer pipe system made of PP or PP filled with mineral material. RAUPIANO PLUS is a sound-absorbing building sewage pipe system and meets the requirements of EN 1451-1 in accordance with the general building supervisory approval. Available pipe dimensions from DN 32 to DN 200 acc. to EN 1451-1 allow for smooth transitions to conventional (not sound-absorbing) PP pipe systems acc. to EN 1451-1 and to sewer pipe systems acc. to EN 1401-1. \n\n\nDue to its three-layer design, RAUPIANO PLUS offers increased pipe stiffness. Number 1 is an abrasive-resistant PP inner layer with very good sliding characteristics. Number 2 consists of a high-stiffness intermediate layer made from mineral-reinforced PP, while number 3 forms an impact-resistant, shock-proof PP outer layer.", "lang": "en"}], "other": {"anies": [{"scenario": [{"description": [{"value": "EoL 100% Deponierung", "lang": "de"}, {"value": "EoL 100% landfilling", "lang": "en"}], "name": "S0", "default": true}, {"description": [{"value": "EoL 100% werkstoffliche Verwertung", "lang": "de"}, {"value": "EoL 100% recycling", "lang": "en"}], "name": "S1"}, {"description": [{"value": "EoL 100% thermische Verwertung", "lang": "de"}, {"value": "EoL 100% energetic utilisation", "lang": "en"}], "name": "S2"}]}]}}, "quantitativeReference": {"referenceToReferenceFlow": [0]}, "time": {"referenceYear": 2024, "dataSetValidUntil": 2029, "other": {"anies": [{"name": "publicationDateOfEPD", "value": 1729555200000}]}}, "geography": {"locationOfOperationSupplyOrProduction": {"location": "GLO"}}, "technology": {"technologyDescriptionAndIncludedProcesses": [{"value": "Die vorliegende Studie bezieht sich auf die Herstellung der kompletten Rohrsysteme, bestehend aus den Rohren, Formteilen in verschiedener Ausführung und den Dichtungsringen, die zwischen den Elementen eingelegt werden. Das Rohrcompound und die Rohre der betrachteten Rohrsysteme werden beim Unternehmen REHAU Industries SE & Co. KG im Werk Velen (Compounds) bzw. Triptis (Rohre), Deutschland produziert. Während der Compoundierung werden dem Polypropylen-Rohmaterial weitere Roh- und Hilfsstoffe, z. B. Stabilisatoren, Pigmente oder Verarbeitungshilfen, hinzugegeben. Die Rohre selbst werden im Extrusionsverfahren hergestellt. Die verschiedenen Formteile werden im Spritzgussverfahren in Viechtach, Deutschland hergestellt. Im ersten Schritt werden Neuwarepolypropylen zusammen mit Pigmenten, Füllstoffen und Hilfsstoffen compoundiert. Im nächsten Schritt erfolgt das Spritzgussverfahren. Beim Spritzguss wird das Polymer plastifiziert und in aufgeschmolzenem Zustand in ein Formwerkzeug gepresst. Zur luft- und wasserdichten Verbindung der Rohre und der Formteile werden Dichtungsringe eingesetzt. Diese werden von REHAU zugekauft. \nTechnische Daten: \nNachfolgend sind die bautechnischen Daten der im Rahmen der Studie betrachteten Produkte in tabellarischer Form dargestellt. \nDeklarierte Einheit: \nAls deklarierte Einheit wird \"1 kg Rohrsystem\" verwendet, das die Komponenten glattes Rohr, Formteil und Dichtungsring umfasst. Eine massenanteilige Aufteilung der Komponenten ist\nin 2.5 dargestellt.\n\nFr die LCA wurde eine Durchschnittsvariante des Rohrsystems RAUPIANO PLUS bilanziert. Es basiert auf den Verkaufsmengen fr das Bezugsjahr 2022 und deckt damit alle Dimensionen und Baulngen ab. Der Massebezug unterscheidet sich je nach Nennweite des Rohres.", "lang": "de"}, {"value": "This study relates to the manufacture of the complete pipe systems, consisting of the pipes, fittings in various designs and the sealing rings that are inserted between the elements. The pipe compound and the pipes of the pipe systems under consideration are manufactured by REHAU Industries SE & Co. KG in Velen (compounds) and Triptis (pipes), Germany. During compounding, further raw materials and additives, e.g. stabilizers, pigments or processing aids, are added to the polypropylene raw material. The pipes themselves are produced using the extrusion process. The various molded parts are produced by injection molding in Viechtach, Germany. In the first step, virgin polypropylene is compounded together with pigments, fillers and additives. The next step is the injection molding process. During injection molding, the polymer is plasticized and pressed into a mould in a molten state. Sealing rings are used to create an airtight and watertight connection between the pipes and the molded parts. These are purchased from REHAU. \nTechnical data: \nThe constructional data of the products assessed in this study is listed in tabular form below. \nDeclared unit: \nThe declared unit is 1 kg pipe system, encompassing the components smooth pipe, fitting, and sealing ring. 2.5 shows the mass fractions of the single components. \n\nAn average variant of the RAUPIANO PLUS pipe system was assessed for the LCA. This is based on the quantities sold in the reference year 2022 and thus covers all dimensions and length. The mass relation varies subject to the pipes dimensions.", "lang": "en"}], "technologicalApplicability": [{"value": "Einsatzbereiche des Rohrsystems sind Entwsserungsanlagen fr Gebude und Grundstcke nach der EN 12056-Reihe im Wohnungsbau (Ein- oder Mehrfamilienhuser und Wohnanlagen), Groprojekte wie z. B. Hotels, Brogebude, Krankenhuser und Schulen, sowie innenliegende Regenwasserleitungen. \nRAUPIANO PLUS besitzt weitere Einsatzbereiche im Bereich der Erdverlegung (innerhalb und unterhalb der Gebudestruktur), als Sammel-, Grund- und Anschlussleitungen sowie in Ein- und Zweifamilienhusern fr dezentrale und zentrale Entlftung von Bdern, Toilettenrumen und Kchen.", "lang": "de"}, {"value": "The pipe system is applied in drainage installations for buildings and properties acc. to the EN 12056 series in the construction of residential buildings (single and multiple dwelling units, housing complexes), large-scale projects such as hotels, office buildings, hospitals and schools, as well as interior rain water lines. \nRAUPIANO PLUS has further applications in the field of buried installations (inside and below building structures), as collecting, ground and connecting line, and in single- and two-family houses for the decentralised and centralised ventilation of bathrooms, toilet rooms, and kitchens.", "lang": "en"}]}}, "modellingAndValidation": {"LCIMethodAndAllocation": {"typeOfDataSet": "EPD", "referenceToLCAMethodDetails": [{"shortDescription": [{"value": "Drucklose Abwasserrohrsysteme aus Kunststoff.pdf", "lang": "de"}], "type": "source data set", "refObjectId": "5bf9ddae-412e-456e-a52f-c02f1bd194f0"}], "other": {"anies": [{"name": "subType", "value": "average dataset"}]}}, "dataSourcesTreatmentAndRepresentativeness": {"referenceToDataSource": [{"shortDescription": [{"value": "GaBi Database (all versions)", "lang": "de"}], "type": "source data set", "refObjectId": "28d74cc0-db8b-4d7e-bc44-5f6d56ce0c4a"}, {"shortDescription": [{"value": "Sphera MLC (fka GaBi) Databases Edition 2024", "lang": "de"}], "type": "source data set", "refObjectId": "7443b962-0446-4d69-8aa7-8055a6b1614a"}], "useAdviceForDataSet": [{"value": "Gültigkeitsbereich: \nInhaber der Deklaration sowie Hersteller des Rohrsystems RAUPIANO PLUS ist das Unternehmen REHAU mit Sitz in Helmut Wagner Strae 1, Rehau.\nDie Herstellung des Compounds fr Formteile und Rohre erfolgt im Werk Velen, die Rohrextrusion findet in Triptis statt, whrend die Herstellung der Formteile im Werk Viechtach erfolgt.\n\nHerstellung der Formteile \nREHAU Industries SE & Co. KG \nSchmidstrae 23 94234 Viechtach\n\nHerstellung der Rohre \nREHAU Industries SE & Co. KG \nIm Klbertale 1 07819 Triptis\n\nHerstellung der Compounds \nREHAU Industries SE & Co. KG \nCoesfelder Str. 47 46342 Velen \nSystemgrenze: \nDer jeweilige Lebenszyklus ist entsprechend DIN EN 15804 modular gestaltet. Die kobilanzen bercksichtigen den Lebenszyklus der Produkte von der Wiege bis zum Werkstor, d. h. A1 - A3 mit den Modulen C1-C4 und Modul D. \n\nIm Folgenden sind die bercksichtigten Lebenswegabschnitte bzw. Prozessmodule des Rohrsystems detailliert aufgelistet: \nA1 – A3 Herstellungsphase\nDieses Modul umfasst die folgenden Prozesse:\n\nProduktion der Roh-, Hilfs- und Betriebsstoffe inkl. Transport zum jeweiligen Werk\nProduktion des Dichtungsrings beim Zulieferer inkl. Transport zum jeweiligen Werk\nProduktion der Verpackungsmaterialien fr das Endprodukt\nEnergiebereitstellung fr die Produktion\nProduktion der Verpackungsmaterialien der Rohstoffe inkl. Transporte zur Verwertung mit anschlieender Verwertung\nTransport der Mehrwegverpackungen der Rohstoffe\nInterne Wiederaufbereitung der Produktionsabflle und Rckfhrung in die Produktion (Umlaufmaterial).C1 – C4 Entsorgung \nEs werden drei 100 %-Entsorgungsszenarien angenommen:\nEnd-of-Life (EoL) Szenario 1 (Deponierung): 100% Rckbau des Rohrsystems mittels Bagger inkl. Transport zum Ort der Entsorgung. Die Entsorgung findet auf einer lokalen Deponie statt (Modul C4 in der Auswertung).\nEoL-Szenario 2 (Recycling): 100% Rckbau des Rohrsystems mittels Bagger inkl. Transport zum Ort der Verwertung mit werkstofflicher Verwertung (Modul C3/2 und D/2 in der Auswertung).\nEoL-Szenario 3 (Energierckgewinnung aus Abfllen): 100% Rckbau des Rohrsystems mittels Bagger inkl. Transport zum Ort der Verwertung mit Energierckgewinnung (Modul C3/1 und D/1 in der Auswertung). \nD Wiederverwendungs-, Rckgewinnungs- und/oder Recyclingpotentiale \nWiederverwendungs-, Rckgewinnungs-, und/oder Recyclingpotentiale sind in den Entsorgungsszenarien vorhanden, da das Rohrsystem einer energetischen bzw. stofflichen Verwertung zugefhrt werden, aus der Energie bzw. Sekundrmaterialien zurckgewonnen werden, die auerhalb der Systemgrenze genutzt werden knnen.", "lang": "de"}, {"value": "Scope: \nThe declaration owner and manufacturer of the pipe system RAUPIANO PLUS is the company REHAU with registered office at Helmut Wagner Strae 1, Rehau. \nThe compound for the fittings and pipes is manufactured in the Velen plant, pipes are extruded in Triptis, and the fittings are manufactured in the Viechtach plant.\n\nProduction of the fittings \nREHAU Industries SE & Co. KG \nSchmidstrae 23 D-94234 Viechtach\n\nProduction of the pipes \nREHAU Industries SE & Co. KG \nIm Klbertale 1 D-07819 Triptis\n\nProduction of the compound \nREHAU Industries SE & Co. KG \nCoesfelder Str. 47 D-46342 Velen \nSystem boundary: \nThe respective life cycle is modular acc. to DIN EN 15804. The life cycle assessments cover the life product life cycle from the cradle to the factory gate, i.e., A1-A3 with modules C1-C4 and module D.\n\nThe life cycle segments or process modules of the pipe system are detailed below: \nA1 – A3 Manufacturing phase\nThis module encompasses the following processes:\n\nProduction of the base, auxiliary and operating materials incl. transport to respective factory\nProduction of the sealing ring at suppliers plant incl. transport to respective factory\nProduction of the packaging materials for the final product\nEnergy supply for production\nProduction of the packaging materials for the raw materials incl. transport to utilisation with subsequent utilisation\nTransport of the reusable packaging of the raw materials \nInternal reprocessing of production waste and feedback into production (circulating material)\nC1 – C4 Disposal\nThree 100% disposal scenarios are assumed:\n\nEnd-of-Life (EoL) scenario 1 (landfilling): 100% deconstruction of the pipe system with excavator incl. transport to disposal site. Disposal takes place at a local landfill (module C4 in the evaluation).\nEoL scenario 2 (recycling): 100% reconstruction of the pipe system with excavator incl. transport to site of utilisation with material utilisation (modules C3/2 and D/2 in the evaluation).\nEoL scenario 3 (energy recovery from waste): 100% reconstruction of the pipe system with excavator incl. transport to site of utilisation with energy recovery (modules C3/1 and D/1 in the evaluation).D Reuse, recovery and/or recycling potentials\nReuse, recovery and/or recycling potentials exist in the disposal scenarios because the pipe system is subjected to energetic or material utilisation with the recovery of energy or secondary materials which can then be used outside the system boundary.", "lang": "en"}], "other": {"anies": [{"name": "referenceToOriginalEPD", "value": {"shortDescription": {"value": "RAUPIANO PLUS.pdf", "defaultValue": "RAUPIANO PLUS.pdf", "lstrings": [{"lang": "de", "value": "RAUPIANO PLUS.pdf"}]}, "type": "source data set", "uuid": {"uuid": "b635d161-8303-4387-ab5d-5a5337869849"}, "refObjectId": "b635d161-8303-4387-ab5d-5a5337869849", "resourceURLs": ["https://oekobaudat.de/OEKOBAU.DAT/resource/sources/b635d161-8303-4387-ab5d-5a5337869849/RAUPIANO_PLUS_23977.pdf?version=00.02.000"]}}]}}, "validation": {"review": [{"referenceToNameOfReviewerAndInstitution": [{"shortDescription": [{"value": "Institut Bauen und Umwelt e. V.", "lang": "de"}], "type": "contact data set", "refObjectId": "d111dbec-b024-4be5-86c5-752d6eb2cf95", "uri": "../contacts/d111dbec-b024-4be5-86c5-752d6eb2cf95.xml"}], "type": "Accredited third party review"}]}, "complianceDeclarations": {"compliance": [{"referenceToComplianceSystem": {"shortDescription": [{"value": "DIN EN 15804+A2", "lang": "de"}], "type": "source data set", "refObjectId": "c0016b33-8cf7-415c-ac6e-deba0d21440d", "uri": "../sources/c0016b33-8cf7-415c-ac6e-deba0d21440d.xml"}}, {"referenceToComplianceSystem": {"shortDescription": [{"value": "ISO 14025", "lang": "de"}], "type": "source data set", "refObjectId": "4f2eb655-6e44-4874-a95a-e28f5442cd4d", "uri": "../sources/4f2eb655-6e44-4874-a95a-e28f5442cd4d.xml"}}]}}, "administrativeInformation": {"commissionerAndGoal": {"referenceToCommissioner": [{"shortDescription": [{"value": "REHAU Industries SE & Co. KG", "lang": "de"}], "type": "contact data set", "refObjectId": "b1b59d51-66a3-4983-acd8-86ad04e48050", "uri": "../contacts/b1b59d51-66a3-4983-acd8-86ad04e48050.xml"}]}, "dataGenerator": {"referenceToPersonOrEntityGeneratingTheDataSet": [{"shortDescription": [{"value": "SKZ - Das Kunststoff-Zentrum", "lang": "de"}], "type": "contact data set", "refObjectId": "2da43b2d-777d-45c6-ba4b-76c55a616a00", "uri": "../contacts/2da43b2d-777d-45c6-ba4b-76c55a616a00.xml"}]}, "dataEntryBy": {"timeStamp": 1729555200000, "referenceToDataSetFormat": [{"shortDescription": [{"value": "ILCD Format", "lang": "de"}], "type": "source data set", "refObjectId": "a97a0155-0234-4b87-b4ce-a45da52f2a40", "uri": "../sources/a97a0155-0234-4b87-b4ce-a45da52f2a40.xml"}, {"shortDescription": [{"value": "EPD-Datenformaterweiterungen v1.2", "lang": "de"}, {"value": "EPD Data Format Extensions v1.2", "lang": "en"}], "type": "source data set", "refObjectId": "a29449fd-aa2f-4de8-b5d7-4b06b43c6fde", "uri": "../sources/a29449fd-aa2f-4de8-b5d7-4b06b43c6fde.xml"}]}, "publicationAndOwnership": {"dataSetVersion": "00.01.200", "referenceToRegistrationAuthority": {"shortDescription": [{"value": "Institut Bauen und Umwelt e. V.", "lang": "de"}], "type": "contact data set", "refObjectId": "d111dbec-b024-4be5-86c5-752d6eb2cf95", "uri": "../contacts/d111dbec-b024-4be5-86c5-752d6eb2cf95.xml"}, "registrationNumber": "EPD-REH-20240258-IBA1-DE", "referenceToOwnershipOfDataSet": {"shortDescription": [{"value": "REHAU Industries SE & Co. KG", "lang": "de"}], "type": "contact data set", "refObjectId": "b1b59d51-66a3-4983-acd8-86ad04e48050", "uri": "../contacts/b1b59d51-66a3-4983-acd8-86ad04e48050.xml"}, "copyright": true, "licenseType": "Free of charge for all users and uses", "accessRestrictions": [{"value": "None", "lang": "en"}], "other": {"anies": [{"name": "referenceToPublisher", "value": {"shortDescription": [{"value": "Institut Bauen und Umwelt e. V.", "lang": "de"}], "type": "contact data set", "refObjectId": "d111dbec-b024-4be5-86c5-752d6eb2cf95", "uri": "../contacts/d111dbec-b024-4be5-86c5-752d6eb2cf95.xml"}}]}}}, "exchanges": {"exchange": [{"dataSetInternalID": 0, "referenceToFlowDataSet": {"shortDescription": [{"value": "RAUPIANO PLUS (RAUPIANO PLUS)", "lang": "de"}], "type": "flow data set", "refObjectId": "51a0c722-bd1d-6ba4-45da-4d0db02c267a", "uri": "../flows/51a0c722-bd1d-6ba4-45da-4d0db02c267a.xml"}, "meanAmount": 1.0, "referencesToDataSource": {}, "referenceFlow": true, "resolvedFlowVersion": "00.01.100", "resultingflowAmount": 1.0, "flowProperties": [{"name": [{"lang": "en", "value": "Mass"}, {"lang": "de", "value": "Masse"}], "uuid": "93a60a56-a3c8-11da-a746-0800200b9a66", "referenceFlowProperty": true, "meanValue": 1.0, "referenceUnit": "kg", "unitGroupUUID": "ad38d542-3fe9-439d-9b95-2f5f7752acaf"}], "materialProperties": [{"name": "gross density", "value": "900.0", "unit": "kg/m^3", "unitDescription": "kilograms per cubic metre"}], "typeOfFlow": "Product flow", "classification": {"classHierarchy": "Kunststoffe / Rohre / Abwasserrohre", "name": "OEKOBAU.DAT"}}, {"dataSetInternalID": 1, "referenceToFlowDataSet": {"shortDescription": [{"value": "Erneuerbare Primärenergie als Energieträger (PERE)", "lang": "de"}, {"value": "Renewable primary energy as energy carrier (PERE)", "lang": "en"}], "type": "flow data set", "refObjectId": "20f32be5-0398-4288-9b6d-accddd195317", "uri": "../flows/20f32be5-0398-4288-9b6d-accddd195317.xml"}, "exchange direction": "INPUT", "other": {"anies": [{"name": "referenceToUnitGroupDataSet", "value": {"shortDescription": [{"value": "MJ", "lang": "de"}], "type": "unit group data set", "refObjectId": "93a60a57-a3c8-11da-a746-0800200c9a66", "uri": "../unitgroups/93a60a57-a3c8-11da-a746-0800200c9a66.xml"}}, {"value": "16.9", "module": "A1-A3"}, {"value": "4.03", "module": "A5"}, {"value": "0.000895", "module": "C1"}, {"value": "0.00548", "module": "C2"}, {"value": "0", "module": "C3", "scenario": "S0"}, {"value": "0.823", "module": "C3", "scenario": "S1"}, {"value": "0.367", "module": "C3", "scenario": "S2"}, {"value": "0.0542", "module": "C4", "scenario": "S0"}, {"value": "0", "module": "C4", "scenario": "S1"}, {"value": "0", "module": "C4", "scenario": "S2"}, {"value": "0", "module": "D", "scenario": "S0"}, {"value": "-1.2", "module": "D", "scenario": "S1"}, {"value": "-3.75", "module": "D", "scenario": "S2"}]}, "resolvedFlowVersion": "38.00.000", "flowProperties": [], "typeOfFlow": "Other flow", "classification": {"classHierarchy": "Quantities", "name": "GaBiCategories"}}, {"dataSetInternalID": 2, "referenceToFlowDataSet": {"shortDescription": [{"value": "Erneuerbare Primärenergie zur stofflichen Nutzung (PERM)", "lang": "de"}, {"value": "Renewable primary energy resources as material utilization (PERM)", "lang": "en"}], "type": "flow data set", "refObjectId": "fb3ec0de-548d-4508-aea5-00b73bf6f702", "uri": "../flows/fb3ec0de-548d-4508-aea5-00b73bf6f702.xml"}, "exchange direction": "INPUT", "other": {"anies": [{"name": "referenceToUnitGroupDataSet", "value": {"shortDescription": [{"value": "MJ", "lang": "de"}], "type": "unit group data set", "refObjectId": "93a60a57-a3c8-11da-a746-0800200c9a66", "uri": "../unitgroups/93a60a57-a3c8-11da-a746-0800200c9a66.xml"}}, {"value": "4.17", "module": "A1-A3"}, {"value": "-3.99", "module": "A5"}, {"value": "0", "module": "C1"}, {"value": "0", "module": "C2"}, {"value": "0", "module": "C3", "scenario": "S0"}, {"value": "-0.173", "module": "C3", "scenario": "S1"}, {"value": "-0.173", "module": "C3", "scenario": "S2"}, {"value": "0", "module": "C4", "scenario": "S0"}, {"value": "0", "module": "C4", "scenario": "S1"}, {"value": "0", "module": "C4", "scenario": "S2"}, {"value": "0", "module": "D", "scenario": "S0"}, {"value": "0", "module": "D", "scenario": "S1"}, {"value": "0", "module": "D", "scenario": "S2"}]}, "resolvedFlowVersion": "38.00.000", "flowProperties": [], "typeOfFlow": "Other flow", "classification": {"classHierarchy": "Quantities", "name": "GaBiCategories"}}, {"dataSetInternalID": 3, "referenceToFlowDataSet": {"shortDescription": [{"value": "Total erneuerbare Primärenergie (PERT)", "lang": "de"}, {"value": "Total use of renewable primary energy resources (PERT)", "lang": "en"}], "type": "flow data set", "refObjectId": "53f97275-fa8a-4cdd-9024-65936002acd0", "uri": "../flows/53f97275-fa8a-4cdd-9024-65936002acd0.xml"}, "exchange direction": "INPUT", "other": {"anies": [{"name": "referenceToUnitGroupDataSet", "value": {"shortDescription": [{"value": "MJ", "lang": "de"}], "type": "unit group data set", "refObjectId": "93a60a57-a3c8-11da-a746-0800200c9a66", "uri": "../unitgroups/93a60a57-a3c8-11da-a746-0800200c9a66.xml"}}, {"value": "21", "module": "A1-A3"}, {"value": "0.0362", "module": "A5"}, {"value": "0.000895", "module": "C1"}, {"value": "0.00548", "module": "C2"}, {"value": "0", "module": "C3", "scenario": "S0"}, {"value": "0.65", "module": "C3", "scenario": "S1"}, {"value": "0.194", "module": "C3", "scenario": "S2"}, {"value": "0.0542", "module": "C4", "scenario": "S0"}, {"value": "0", "module": "C4", "scenario": "S1"}, {"value": "0", "module": "C4", "scenario": "S2"}, {"value": "0", "module": "D", "scenario": "S0"}, {"value": "-1.2", "module": "D", "scenario": "S1"}, {"value": "-3.75", "module": "D", "scenario": "S2"}]}, "resolvedFlowVersion": "38.00.000", "flowProperties": [], "typeOfFlow": "Other flow", "classification": {"classHierarchy": "Quantities / Environmental quantities / EPD EN 15804 / LCI indicators", "name": "GaBiCategories"}}, {"dataSetInternalID": 4, "referenceToFlowDataSet": {"shortDescription": [{"value": "Nicht-erneuerbare Primärenergie als Energieträger (PENRE)", "lang": "de"}, {"value": "Non renewable primary energy as energy carrier (PENRE)", "lang": "en"}], "type": "flow data set", "refObjectId": "ac857178-2b45-46ec-892a-a9a4332f0372", "uri": "../flows/ac857178-2b45-46ec-892a-a9a4332f0372.xml"}, "exchange direction": "INPUT", "other": {"anies": [{"name": "referenceToUnitGroupDataSet", "value": {"shortDescription": [{"value": "MJ", "lang": "de"}], "type": "unit group data set", "refObjectId": "93a60a57-a3c8-11da-a746-0800200c9a66", "uri": "../unitgroups/93a60a57-a3c8-11da-a746-0800200c9a66.xml"}}, {"value": "43.3", "module": "A1-A3"}, {"value": "1.68", "module": "A5"}, {"value": "0.00809", "module": "C1"}, {"value": "0.0495", "module": "C2"}, {"value": "0", "module": "C3", "scenario": "S0"}, {"value": "3.29", "module": "C3", "scenario": "S1"}, {"value": "21.4", "module": "C3", "scenario": "S2"}, {"value": "0.343", "module": "C4", "scenario": "S0"}, {"value": "0", "module": "C4", "scenario": "S1"}, {"value": "0", "module": "C4", "scenario": "S2"}, {"value": "0", "module": "D", "scenario": "S0"}, {"value": "-17.5", "module": "D", "scenario": "S1"}, {"value": "-11.8", "module": "D", "scenario": "S2"}]}, "resolvedFlowVersion": "38.00.000", "flowProperties": [], "typeOfFlow": "Other flow", "classification": {"classHierarchy": "Quantities", "name": "GaBiCategories"}}, {"dataSetInternalID": 5, "referenceToFlowDataSet": {"shortDescription": [{"value": "Nicht-erneuerbare Primärenergie zur stofflichen Nutzung (PENRM)", "lang": "de"}, {"value": "Non renewable primary energy as material utilization (PENRM)", "lang": "en"}], "type": "flow data set", "refObjectId": "1421caa0-679d-4bf4-b282-0eb850ccae27", "uri": "../flows/1421caa0-679d-4bf4-b282-0eb850ccae27.xml"}, "exchange direction": "INPUT", "other": {"anies": [{"name": "referenceToUnitGroupDataSet", "value": {"shortDescription": [{"value": "MJ", "lang": "de"}], "type": "unit group data set", "refObjectId": "93a60a57-a3c8-11da-a746-0800200c9a66", "uri": "../unitgroups/93a60a57-a3c8-11da-a746-0800200c9a66.xml"}}, {"value": "18.5", "module": "A1-A3"}, {"value": "-1.55", "module": "A5"}, {"value": "0", "module": "C1"}, {"value": "0", "module": "C2"}, {"value": "0", "module": "C3", "scenario": "S0"}, {"value": "-16.9", "module": "C3", "scenario": "S1"}, {"value": "-16.9", "module": "C3", "scenario": "S2"}, {"value": "0", "module": "C4", "scenario": "S0"}, {"value": "0", "module": "C4", "scenario": "S1"}, {"value": "0", "module": "C4", "scenario": "S2"}, {"value": "0", "module": "D", "scenario": "S0"}, {"value": "0", "module": "D", "scenario": "S1"}, {"value": "0", "module": "D", "scenario": "S2"}]}, "resolvedFlowVersion": "38.00.000", "flowProperties": [], "typeOfFlow": "Other flow", "classification": {"classHierarchy": "Quantities", "name": "GaBiCategories"}}, {"dataSetInternalID": 6, "referenceToFlowDataSet": {"shortDescription": [{"value": "Total nicht erneuerbare Primärenergie (PENRT)", "lang": "de"}, {"value": "Total use of non renewable primary energy resources (PENRT)", "lang": "en"}], "type": "flow data set", "refObjectId": "06159210-646b-4c8d-8583-da9b3b95a6c1", "uri": "../flows/06159210-646b-4c8d-8583-da9b3b95a6c1.xml"}, "exchange direction": "INPUT", "other": {"anies": [{"name": "referenceToUnitGroupDataSet", "value": {"shortDescription": [{"value": "MJ", "lang": "de"}], "type": "unit group data set", "refObjectId": "93a60a57-a3c8-11da-a746-0800200c9a66", "uri": "../unitgroups/93a60a57-a3c8-11da-a746-0800200c9a66.xml"}}, {"value": "61.8", "module": "A1-A3"}, {"value": "0.13", "module": "A5"}, {"value": "0.00809", "module": "C1"}, {"value": "0.0495", "module": "C2"}, {"value": "0", "module": "C3", "scenario": "S0"}, {"value": "-13.6", "module": "C3", "scenario": "S1"}, {"value": "4.49", "module": "C3", "scenario": "S2"}, {"value": "0.343", "module": "C4", "scenario": "S0"}, {"value": "0", "module": "C4", "scenario": "S1"}, {"value": "0", "module": "C4", "scenario": "S2"}, {"value": "0", "module": "D", "scenario": "S0"}, {"value": "-17.5", "module": "D", "scenario": "S1"}, {"value": "-11.8", "module": "D", "scenario": "S2"}]}, "resolvedFlowVersion": "38.00.000", "flowProperties": [], "typeOfFlow": "Other flow", "classification": {"classHierarchy": "Quantities / Environmental quantities / EPD EN 15804 / LCI indicators", "name": "GaBiCategories"}}, {"dataSetInternalID": 7, "referenceToFlowDataSet": {"shortDescription": [{"value": "Einsatz von Sekundärstoffen (SM)", "lang": "de"}, {"value": "Use of secondary material (SM)", "lang": "en"}], "type": "flow data set", "refObjectId": "c6a1f35f-2d09-4f54-8dfb-97e502e1ce92", "uri": "../flows/c6a1f35f-2d09-4f54-8dfb-97e502e1ce92.xml"}, "exchange direction": "INPUT", "other": {"anies": [{"name": "referenceToUnitGroupDataSet", "value": {"shortDescription": [{"value": "kg", "lang": "de"}], "type": "unit group data set", "refObjectId": "ad38d542-3fe9-439d-9b95-2f5f7752acaf", "uri": "../unitgroups/ad38d542-3fe9-439d-9b95-2f5f7752acaf.xml"}}, {"value": "0", "module": "A1-A3"}, {"value": "0", "module": "A5"}, {"value": "0", "module": "C1"}, {"value": "0", "module": "C2"}, {"value": "0", "module": "C3", "scenario": "S0"}, {"value": "0", "module": "C3", "scenario": "S1"}, {"value": "0", "module": "C3", "scenario": "S2"}, {"value": "0", "module": "C4", "scenario": "S0"}, {"value": "0", "module": "C4", "scenario": "S1"}, {"value": "0", "module": "C4", "scenario": "S2"}, {"value": "0", "module": "D", "scenario": "S0"}, {"value": "0.95", "module": "D", "scenario": "S1"}, {"value": "0", "module": "D", "scenario": "S2"}]}, "resolvedFlowVersion": "38.00.000", "flowProperties": [], "typeOfFlow": "Other flow", "classification": {"classHierarchy": "Quantities / Environmental quantities / EPD EN 15804 / LCI indicators", "name": "GaBiCategories"}}, {"dataSetInternalID": 8, "referenceToFlowDataSet": {"shortDescription": [{"value": "Erneuerbare Sekundärbrennstoffe (RSF)", "lang": "de"}, {"value": "Use of renewable secondary fuels (RSF)", "lang": "en"}], "type": "flow data set", "refObjectId": "64333088-a55f-4aa2-9a31-c10b07816787", "uri": "../flows/64333088-a55f-4aa2-9a31-c10b07816787.xml"}, "exchange direction": "INPUT", "other": {"anies": [{"name": "referenceToUnitGroupDataSet", "value": {"shortDescription": [{"value": "MJ", "lang": "de"}], "type": "unit group data set", "refObjectId": "93a60a57-a3c8-11da-a746-0800200c9a66", "uri": "../unitgroups/93a60a57-a3c8-11da-a746-0800200c9a66.xml"}}, {"value": "0", "module": "A1-A3"}, {"value": "0", "module": "A5"}, {"value": "0", "module": "C1"}, {"value": "0", "module": "C2"}, {"value": "0", "module": "C3", "scenario": "S0"}, {"value": "0", "module": "C3", "scenario": "S1"}, {"value": "0", "module": "C3", "scenario": "S2"}, {"value": "0", "module": "C4", "scenario": "S0"}, {"value": "0", "module": "C4", "scenario": "S1"}, {"value": "0", "module": "C4", "scenario": "S2"}, {"value": "0", "module": "D", "scenario": "S0"}, {"value": "0", "module": "D", "scenario": "S1"}, {"value": "0", "module": "D", "scenario": "S2"}]}, "resolvedFlowVersion": "38.00.000", "flowProperties": [], "typeOfFlow": "Other flow", "classification": {"classHierarchy": "Quantities / Environmental quantities / EPD EN 15804 / LCI indicators", "name": "GaBiCategories"}}, {"dataSetInternalID": 9, "referenceToFlowDataSet": {"shortDescription": [{"value": "Nicht erneuerbare Sekundärbrennstoffe (NRSF)", "lang": "de"}, {"value": "Use of non renewable secondary fuels (NRSF)", "lang": "en"}], "type": "flow data set", "refObjectId": "89def144-d39a-4287-b86f-efde453ddcb2", "uri": "../flows/89def144-d39a-4287-b86f-efde453ddcb2.xml"}, "exchange direction": "INPUT", "other": {"anies": [{"name": "referenceToUnitGroupDataSet", "value": {"shortDescription": [{"value": "MJ", "lang": "de"}], "type": "unit group data set", "refObjectId": "93a60a57-a3c8-11da-a746-0800200c9a66", "uri": "../unitgroups/93a60a57-a3c8-11da-a746-0800200c9a66.xml"}}, {"value": "0", "module": "A1-A3"}, {"value": "0", "module": "A5"}, {"value": "0", "module": "C1"}, {"value": "0", "module": "C2"}, {"value": "0", "module": "C3", "scenario": "S0"}, {"value": "0", "module": "C3", "scenario": "S1"}, {"value": "0", "module": "C3", "scenario": "S2"}, {"value": "0", "module": "C4", "scenario": "S0"}, {"value": "0", "module": "C4", "scenario": "S1"}, {"value": "0", "module": "C4", "scenario": "S2"}, {"value": "0", "module": "D", "scenario": "S0"}, {"value": "0", "module": "D", "scenario": "S1"}, {"value": "0", "module": "D", "scenario": "S2"}]}, "resolvedFlowVersion": "38.00.000", "flowProperties": [], "typeOfFlow": "Other flow", "classification": {"classHierarchy": "Quantities / Environmental quantities / EPD EN 15804 / LCI indicators", "name": "GaBiCategories"}}, {"dataSetInternalID": 10, "referenceToFlowDataSet": {"shortDescription": [{"value": "Einsatz von Süßwasserressourcen (FW)", "lang": "de"}, {"value": "Use of net fresh water (FW)", "lang": "en"}], "type": "flow data set", "refObjectId": "3cf952c8-f3a4-461d-8c96-96456ca62246", "uri": "../flows/3cf952c8-f3a4-461d-8c96-96456ca62246.xml"}, "exchange direction": "INPUT", "other": {"anies": [{"name": "referenceToUnitGroupDataSet", "value": {"shortDescription": [{"value": "m^3", "lang": "de"}], "type": "unit group data set", "refObjectId": "cd950537-0a98-4044-9ba7-9f9a68d0a504", "uri": "../unitgroups/cd950537-0a98-4044-9ba7-9f9a68d0a504.xml"}}, {"value": "0.0186", "module": "A1-A3"}, {"value": "0.00122", "module": "A5"}, {"value": "8.36E-07", "module": "C1"}, {"value": "5.12E-06", "module": "C2"}, {"value": "0", "module": "C3", "scenario": "S0"}, {"value": "0.00195", "module": "C3", "scenario": "S1"}, {"value": "0.00471", "module": "C3", "scenario": "S2"}, {"value": "8.2E-05", "module": "C4", "scenario": "S0"}, {"value": "0", "module": "C4", "scenario": "S1"}, {"value": "0", "module": "C4", "scenario": "S2"}, {"value": "0", "module": "D", "scenario": "S0"}, {"value": "-0.00205", "module": "D", "scenario": "S1"}, {"value": "-0.00288", "module": "D", "scenario": "S2"}]}, "resolvedFlowVersion": "38.00.000", "flowProperties": [], "typeOfFlow": "Other flow", "classification": {"classHierarchy": "Quantities / Environmental quantities / EPD EN 15804 / LCI indicators", "name": "GaBiCategories"}}, {"dataSetInternalID": 11, "referenceToFlowDataSet": {"shortDescription": [{"value": "Gefährlicher Abfall zur Deponie (HWD)", "lang": "de"}, {"value": "Hazardous waste disposed (HWD)", "lang": "en"}], "type": "flow data set", "refObjectId": "430f9e0f-59b2-46a0-8e0d-55e0e84948fc", "uri": "../flows/430f9e0f-59b2-46a0-8e0d-55e0e84948fc.xml"}, "exchange direction": "OUTPUT", "other": {"anies": [{"name": "referenceToUnitGroupDataSet", "value": {"shortDescription": [{"value": "kg", "lang": "de"}], "type": "unit group data set", "refObjectId": "ad38d542-3fe9-439d-9b95-2f5f7752acaf", "uri": "../unitgroups/ad38d542-3fe9-439d-9b95-2f5f7752acaf.xml"}}, {"value": "4.07E-08", "module": "A1-A3"}, {"value": "7.63E-11", "module": "A5"}, {"value": "3.94E-13", "module": "C1"}, {"value": "2.41E-12", "module": "C2"}, {"value": "0", "module": "C3", "scenario": "S0"}, {"value": "1.62E-09", "module": "C3", "scenario": "S1"}, {"value": "4.22E-10", "module": "C3", "scenario": "S2"}, {"value": "8.51E-11", "module": "C4", "scenario": "S0"}, {"value": "0", "module": "C4", "scenario": "S1"}, {"value": "0", "module": "C4", "scenario": "S2"}, {"value": "0", "module": "D", "scenario": "S0"}, {"value": "-2.78E-09", "module": "D", "scenario": "S1"}, {"value": "-7.62E-09", "module": "D", "scenario": "S2"}]}, "resolvedFlowVersion": "38.00.000", "flowProperties": [], "typeOfFlow": "Other flow", "classification": {"classHierarchy": "Quantities / Environmental quantities / EPD EN 15804 / LCI indicators", "name": "GaBiCategories"}}, {"dataSetInternalID": 12, "referenceToFlowDataSet": {"shortDescription": [{"value": "Entsorgter nicht gefährlicher Abfall (NHWD)", "lang": "de"}, {"value": "Non hazardous waste disposed (NHWD)", "lang": "en"}], "type": "flow data set", "refObjectId": "b29ef66b-e286-4afa-949f-62f1a7b4d7fa", "uri": "../flows/b29ef66b-e286-4afa-949f-62f1a7b4d7fa.xml"}, "exchange direction": "OUTPUT", "other": {"anies": [{"name": "referenceToUnitGroupDataSet", "value": {"shortDescription": [{"value": "kg", "lang": "de"}], "type": "unit group data set", "refObjectId": "ad38d542-3fe9-439d-9b95-2f5f7752acaf", "uri": "../unitgroups/ad38d542-3fe9-439d-9b95-2f5f7752acaf.xml"}}, {"value": "0.0365", "module": "A1-A3"}, {"value": "0.00598", "module": "A5"}, {"value": "1.37E-06", "module": "C1"}, {"value": "8.37E-06", "module": "C2"}, {"value": "0", "module": "C3", "scenario": "S0"}, {"value": "0.00186", "module": "C3", "scenario": "S1"}, {"value": "0.0775", "module": "C3", "scenario": "S2"}, {"value": "0.998", "module": "C4", "scenario": "S0"}, {"value": "0", "module": "C4", "scenario": "S1"}, {"value": "0", "module": "C4", "scenario": "S2"}, {"value": "0", "module": "D", "scenario": "S0"}, {"value": "-0.00447", "module": "D", "scenario": "S1"}, {"value": "-0.00563", "module": "D", "scenario": "S2"}]}, "resolvedFlowVersion": "38.00.000", "flowProperties": [], "typeOfFlow": "Other flow", "classification": {"classHierarchy": "Quantities / Environmental quantities / EPD EN 15804 / LCI indicators", "name": "GaBiCategories"}}, {"dataSetInternalID": 13, "referenceToFlowDataSet": {"shortDescription": [{"value": "Entsorgter radioaktiver Abfall (RWD)", "lang": "de"}, {"value": "Radioactive waste disposed (RWD)", "lang": "en"}], "type": "flow data set", "refObjectId": "3449546e-52ad-4b39-b809-9fb77cea8ff6", "uri": "../flows/3449546e-52ad-4b39-b809-9fb77cea8ff6.xml"}, "exchange direction": "OUTPUT", "other": {"anies": [{"name": "referenceToUnitGroupDataSet", "value": {"shortDescription": [{"value": "kg", "lang": "de"}], "type": "unit group data set", "refObjectId": "ad38d542-3fe9-439d-9b95-2f5f7752acaf", "uri": "../unitgroups/ad38d542-3fe9-439d-9b95-2f5f7752acaf.xml"}}, {"value": "0.000491", "module": "A1-A3"}, {"value": "4.42E-06", "module": "A5"}, {"value": "1.29E-08", "module": "C1"}, {"value": "7.88E-08", "module": "C2"}, {"value": "0", "module": "C3", "scenario": "S0"}, {"value": "0.000179", "module": "C3", "scenario": "S1"}, {"value": "2.23E-05", "module": "C3", "scenario": "S2"}, {"value": "4.45E-06", "module": "C4", "scenario": "S0"}, {"value": "0", "module": "C4", "scenario": "S1"}, {"value": "0", "module": "C4", "scenario": "S2"}, {"value": "0", "module": "D", "scenario": "S0"}, {"value": "-0.000178", "module": "D", "scenario": "S1"}, {"value": "-0.000827", "module": "D", "scenario": "S2"}]}, "resolvedFlowVersion": "38.00.000", "flowProperties": [], "typeOfFlow": "Other flow", "classification": {"classHierarchy": "Quantities / Environmental quantities / EPD EN 15804 / LCI indicators", "name": "GaBiCategories"}}, {"dataSetInternalID": 14, "referenceToFlowDataSet": {"shortDescription": [{"value": "Komponenten für die Wiederverwendung (CRU)", "lang": "de"}, {"value": "Components for re-use (CRU)", "lang": "en"}], "type": "flow data set", "refObjectId": "a2b32f97-3fc7-4af2-b209-525bc6426f33", "uri": "../flows/a2b32f97-3fc7-4af2-b209-525bc6426f33.xml"}, "exchange direction": "OUTPUT", "other": {"anies": [{"name": "referenceToUnitGroupDataSet", "value": {"shortDescription": [{"value": "kg", "lang": "de"}], "type": "unit group data set", "refObjectId": "ad38d542-3fe9-439d-9b95-2f5f7752acaf", "uri": "../unitgroups/ad38d542-3fe9-439d-9b95-2f5f7752acaf.xml"}}, {"value": "0", "module": "A1-A3"}, {"value": "0", "module": "A5"}, {"value": "0", "module": "C1"}, {"value": "0", "module": "C2"}, {"value": "0", "module": "C3", "scenario": "S0"}, {"value": "0", "module": "C3", "scenario": "S1"}, {"value": "0", "module": "C3", "scenario": "S2"}, {"value": "0", "module": "C4", "scenario": "S0"}, {"value": "0", "module": "C4", "scenario": "S1"}, {"value": "0", "module": "C4", "scenario": "S2"}, {"value": "0", "module": "D", "scenario": "S0"}, {"value": "0", "module": "D", "scenario": "S1"}, {"value": "0", "module": "D", "scenario": "S2"}]}, "resolvedFlowVersion": "38.00.000", "flowProperties": [], "typeOfFlow": "Other flow", "classification": {"classHierarchy": "Quantities / Environmental quantities / EPD EN 15804 / LCI indicators", "name": "GaBiCategories"}}, {"dataSetInternalID": 15, "referenceToFlowDataSet": {"shortDescription": [{"value": "Stoffe zum Recycling (MFR)", "lang": "de"}, {"value": "Materials for recycling (MFR)", "lang": "en"}], "type": "flow data set", "refObjectId": "d7fe48a5-4103-49c8-9aae-b0b5dfdbd6ae", "uri": "../flows/d7fe48a5-4103-49c8-9aae-b0b5dfdbd6ae.xml"}, "exchange direction": "OUTPUT", "other": {"anies": [{"name": "referenceToUnitGroupDataSet", "value": {"shortDescription": [{"value": "kg", "lang": "de"}], "type": "unit group data set", "refObjectId": "ad38d542-3fe9-439d-9b95-2f5f7752acaf", "uri": "../unitgroups/ad38d542-3fe9-439d-9b95-2f5f7752acaf.xml"}}, {"value": "0.111", "module": "A1-A3"}, {"value": "0", "module": "A5"}, {"value": "0", "module": "C1"}, {"value": "0", "module": "C2"}, {"value": "0", "module": "C3", "scenario": "S0"}, {"value": "1", "module": "C3", "scenario": "S1"}, {"value": "0", "module": "C3", "scenario": "S2"}, {"value": "0", "module": "C4", "scenario": "S0"}, {"value": "0", "module": "C4", "scenario": "S1"}, {"value": "0", "module": "C4", "scenario": "S2"}, {"value": "0", "module": "D", "scenario": "S0"}, {"value": "0", "module": "D", "scenario": "S1"}, {"value": "0", "module": "D", "scenario": "S2"}]}, "resolvedFlowVersion": "38.00.000", "flowProperties": [], "typeOfFlow": "Other flow", "classification": {"classHierarchy": "Quantities / Environmental quantities / EPD EN 15804 / LCI indicators", "name": "GaBiCategories"}}, {"dataSetInternalID": 16, "referenceToFlowDataSet": {"shortDescription": [{"value": "Stoffe für die Energierückgewinnung (MER)", "lang": "de"}, {"value": "Materials for energy recovery (MER)", "lang": "en"}], "type": "flow data set", "refObjectId": "59a9181c-3aaf-46ee-8b13-2b3723b6e447", "uri": "../flows/59a9181c-3aaf-46ee-8b13-2b3723b6e447.xml"}, "exchange direction": "OUTPUT", "other": {"anies": [{"name": "referenceToUnitGroupDataSet", "value": {"shortDescription": [{"value": "kg", "lang": "de"}], "type": "unit group data set", "refObjectId": "ad38d542-3fe9-439d-9b95-2f5f7752acaf", "uri": "../unitgroups/ad38d542-3fe9-439d-9b95-2f5f7752acaf.xml"}}, {"value": "0", "module": "A1-A3"}, {"value": "0", "module": "A5"}, {"value": "0", "module": "C1"}, {"value": "0", "module": "C2"}, {"value": "0", "module": "C3", "scenario": "S0"}, {"value": "0", "module": "C3", "scenario": "S1"}, {"value": "0", "module": "C3", "scenario": "S2"}, {"value": "0", "module": "C4", "scenario": "S0"}, {"value": "0", "module": "C4", "scenario": "S1"}, {"value": "0", "module": "C4", "scenario": "S2"}, {"value": "0", "module": "D", "scenario": "S0"}, {"value": "0", "module": "D", "scenario": "S1"}, {"value": "0", "module": "D", "scenario": "S2"}]}, "resolvedFlowVersion": "38.00.000", "flowProperties": [], "typeOfFlow": "Other flow", "classification": {"classHierarchy": "Quantities / Environmental quantities / EPD EN 15804 / LCI indicators", "name": "GaBiCategories"}}, {"dataSetInternalID": 17, "referenceToFlowDataSet": {"shortDescription": [{"value": "Exportierte elektrische Energie (EEE)", "lang": "de"}, {"value": "Exported electrical energy (EEE)", "lang": "en"}], "type": "flow data set", "refObjectId": "4da0c987-2b76-40d6-9e9e-82a017aaaf29", "uri": "../flows/4da0c987-2b76-40d6-9e9e-82a017aaaf29.xml"}, "exchange direction": "OUTPUT", "other": {"anies": [{"name": "referenceToUnitGroupDataSet", "value": {"shortDescription": [{"value": "MJ", "lang": "de"}], "type": "unit group data set", "refObjectId": "93a60a57-a3c8-11da-a746-0800200c9a66", "uri": "../unitgroups/93a60a57-a3c8-11da-a746-0800200c9a66.xml"}}, {"value": "0.0476", "module": "A1-A3"}, {"value": "0.739", "module": "A5"}, {"value": "0", "module": "C1"}, {"value": "0", "module": "C2"}, {"value": "0", "module": "C3", "scenario": "S0"}, {"value": "0.334", "module": "C3", "scenario": "S1"}, {"value": "3.08", "module": "C3", "scenario": "S2"}, {"value": "0", "module": "C4", "scenario": "S0"}, {"value": "0", "module": "C4", "scenario": "S1"}, {"value": "0", "module": "C4", "scenario": "S2"}, {"value": "0", "module": "D", "scenario": "S0"}, {"value": "0", "module": "D", "scenario": "S1"}, {"value": "0", "module": "D", "scenario": "S2"}]}, "resolvedFlowVersion": "38.00.000", "flowProperties": [], "typeOfFlow": "Other flow", "classification": {"classHierarchy": "Quantities / Environmental quantities / EPD EN 15804 / LCI indicators", "name": "GaBiCategories"}}, {"dataSetInternalID": 18, "referenceToFlowDataSet": {"shortDescription": [{"value": "Exportierte thermische Energie (EET)", "lang": "de"}, {"value": "Exported thermal energy (EET)", "lang": "en"}], "type": "flow data set", "refObjectId": "98daf38a-7a79-46d3-9a37-2b7bd0955810", "uri": "../flows/98daf38a-7a79-46d3-9a37-2b7bd0955810.xml"}, "exchange direction": "OUTPUT", "other": {"anies": [{"name": "referenceToUnitGroupDataSet", "value": {"shortDescription": [{"value": "MJ", "lang": "de"}], "type": "unit group data set", "refObjectId": "93a60a57-a3c8-11da-a746-0800200c9a66", "uri": "../unitgroups/93a60a57-a3c8-11da-a746-0800200c9a66.xml"}}, {"value": "0.111", "module": "A1-A3"}, {"value": "1.5", "module": "A5"}, {"value": "0", "module": "C1"}, {"value": "0", "module": "C2"}, {"value": "0", "module": "C3", "scenario": "S0"}, {"value": "0.594", "module": "C3", "scenario": "S1"}, {"value": "5.57", "module": "C3", "scenario": "S2"}, {"value": "0", "module": "C4", "scenario": "S0"}, {"value": "0", "module": "C4", "scenario": "S1"}, {"value": "0", "module": "C4", "scenario": "S2"}, {"value": "0", "module": "D", "scenario": "S0"}, {"value": "0", "module": "D", "scenario": "S1"}, {"value": "0", "module": "D", "scenario": "S2"}]}, "resolvedFlowVersion": "38.00.000", "flowProperties": [], "typeOfFlow": "Other flow", "classification": {"classHierarchy": "Quantities / Environmental quantities / EPD EN 15804 / LCI indicators", "name": "GaBiCategories"}}]}, "LCIAResults": {"LCIAResult": [{"referenceToLCIAMethodDataSet": {"shortDescription": [{"value": "Globales Erwärmungspotenzial total (GWP-total)", "lang": "de"}, {"value": "Global Warming Potential total (GWP-total)", "lang": "en"}], "type": "LCIA method data set", "refObjectId": "6a37f984-a4b3-458a-a20a-64418c145fa2", "uri": "../lciamethods/6a37f984-a4b3-458a-a20a-64418c145fa2.xml"}, "other": {"anies": [{"name": "referenceToUnitGroupDataSet", "value": {"shortDescription": [{"value": "kg CO_(2)-Äq.", "lang": "de"}], "type": "unit group data set", "refObjectId": "1ebf3012-d0db-4de2-aefd-ef30cedb0be1", "uri": "../unitgroups/1ebf3012-d0db-4de2-aefd-ef30cedb0be1.xml"}}, {"value": "1.39", "module": "A1-A3"}, {"value": "0.495", "module": "A5"}, {"value": "0.00064", "module": "C1"}, {"value": "0.00387", "module": "C2"}, {"value": "0", "module": "C3", "scenario": "S0"}, {"value": "0.219778326374832", "module": "C3", "scenario": "S1"}, {"value": "1.56258186451954", "module": "C3", "scenario": "S2"}, {"value": "0.0312029469345089", "module": "C4", "scenario": "S0"}, {"value": "0", "module": "C4", "scenario": "S1"}, {"value": "0", "module": "C4", "scenario": "S2"}, {"value": "0", "module": "D", "scenario": "S0"}, {"value": "-0.543", "module": "D", "scenario": "S1"}, {"value": "-0.759", "module": "D", "scenario": "S2"}]}}, {"referenceToLCIAMethodDataSet": {"shortDescription": [{"value": "Globales Erwärmungspotenzial fossil (GWP-fossil)", "lang": "de"}, {"value": "Global Warming Potential fossil fuels (GWP-fossil)", "lang": "en"}], "type": "LCIA method data set", "refObjectId": "5f635281-343e-44fb-83df-1971b155e6b6", "uri": "../lciamethods/5f635281-343e-44fb-83df-1971b155e6b6.xml"}, "other": {"anies": [{"name": "referenceToUnitGroupDataSet", "value": {"shortDescription": [{"value": "kg CO_(2)-Äq.", "lang": "de"}], "type": "unit group data set", "refObjectId": "1ebf3012-d0db-4de2-aefd-ef30cedb0be1", "uri": "../unitgroups/1ebf3012-d0db-4de2-aefd-ef30cedb0be1.xml"}}, {"value": "1.72", "module": "A1-A3"}, {"value": "0.121", "module": "A5"}, {"value": "0.000646", "module": "C1"}, {"value": "0.00377", "module": "C2"}, {"value": "0", "module": "C3", "scenario": "S0"}, {"value": "0.21", "module": "C3", "scenario": "S1"}, {"value": "1.55", "module": "C3", "scenario": "S2"}, {"value": "0.022", "module": "C4", "scenario": "S0"}, {"value": "0", "module": "C4", "scenario": "S1"}, {"value": "0", "module": "C4", "scenario": "S2"}, {"value": "0", "module": "D", "scenario": "S0"}, {"value": "-0.54", "module": "D", "scenario": "S1"}, {"value": "-0.756", "module": "D", "scenario": "S2"}]}}, {"referenceToLCIAMethodDataSet": {"shortDescription": [{"value": "Globales Erwärmungspotenzial biogen (GWP-biogenic)", "lang": "de"}, {"value": "Global Warming Potential biogenic (GWP-biogenic)", "lang": "en"}], "type": "LCIA method data set", "refObjectId": "2356e1ab-0185-4db5-86e5-16de51c7485c", "uri": "../lciamethods/2356e1ab-0185-4db5-86e5-16de51c7485c.xml"}, "other": {"anies": [{"name": "referenceToUnitGroupDataSet", "value": {"shortDescription": [{"value": "kg CO_(2)-Äq.", "lang": "de"}], "type": "unit group data set", "refObjectId": "1ebf3012-d0db-4de2-aefd-ef30cedb0be1", "uri": "../unitgroups/1ebf3012-d0db-4de2-aefd-ef30cedb0be1.xml"}}, {"value": "-0.338", "module": "A1-A3"}, {"value": "0.374", "module": "A5"}, {"value": "0", "module": "C1"}, {"value": "2.16E-05", "module": "C2"}, {"value": "0", "module": "C3", "scenario": "S0"}, {"value": "0.00961857536978357", "module": "C3", "scenario": "S1"}, {"value": "0.00916303720905496", "module": "C3", "scenario": "S2"}, {"value": "0.00912268091805518", "module": "C4", "scenario": "S0"}, {"value": "0", "module": "C4", "scenario": "S1"}, {"value": "0", "module": "C4", "scenario": "S2"}, {"value": "0", "module": "D", "scenario": "S0"}, {"value": "-0.00263", "module": "D", "scenario": "S1"}, {"value": "-0.0027", "module": "D", "scenario": "S2"}]}}, {"referenceToLCIAMethodDataSet": {"shortDescription": [{"value": "Globales Erwärmungspotenzial luluc (GWP-luluc)", "lang": "de"}, {"value": "Global Warming Potential luluc (GWP-luluc)", "lang": "en"}], "type": "LCIA method data set", "refObjectId": "4331bbdb-978a-490d-8707-eeb047f01a55", "uri": "../lciamethods/4331bbdb-978a-490d-8707-eeb047f01a55.xml"}, "other": {"anies": [{"name": "referenceToUnitGroupDataSet", "value": {"shortDescription": [{"value": "kg CO_(2)-Äq.", "lang": "de"}], "type": "unit group data set", "refObjectId": "1ebf3012-d0db-4de2-aefd-ef30cedb0be1", "uri": "../unitgroups/1ebf3012-d0db-4de2-aefd-ef30cedb0be1.xml"}}, {"value": "0.00262", "module": "A1-A3"}, {"value": "3.53E-05", "module": "A5"}, {"value": "1.18E-05", "module": "C1"}, {"value": "7.25E-05", "module": "C2"}, {"value": "0", "module": "C3", "scenario": "S0"}, {"value": "1.22E-05", "module": "C3", "scenario": "S1"}, {"value": "0.000118", "module": "C3", "scenario": "S2"}, {"value": "9.88E-05", "module": "C4", "scenario": "S0"}, {"value": "0", "module": "C4", "scenario": "S1"}, {"value": "0", "module": "C4", "scenario": "S2"}, {"value": "0", "module": "D", "scenario": "S0"}, {"value": "-0.000115", "module": "D", "scenario": "S1"}, {"value": "-5.58E-05", "module": "D", "scenario": "S2"}]}}, {"referenceToLCIAMethodDataSet": {"shortDescription": [{"value": "Abbau Potential der stratosphärischen Ozonschicht (ODP)", "lang": "de"}, {"value": "Depletion potential of the stratospheric ozone layer (ODP)", "lang": "en"}], "type": "LCIA method data set", "refObjectId": "b5c629d6-def3-11e6-bf01-fe55135034f3", "uri": "../lciamethods/b5c629d6-def3-11e6-bf01-fe55135034f3.xml"}, "other": {"anies": [{"name": "referenceToUnitGroupDataSet", "value": {"shortDescription": [{"value": "kg CFC11-Äq.", "lang": "de"}], "type": "unit group data set", "refObjectId": "d9e957c9-7309-4474-bf3a-7777df6c4e5b", "uri": "../unitgroups/d9e957c9-7309-4474-bf3a-7777df6c4e5b.xml"}}, {"value": "2.45E-11", "module": "A1-A3"}, {"value": "6.43E-14", "module": "A5"}, {"value": "1.94E-16", "module": "C1"}, {"value": "1.19E-15", "module": "C2"}, {"value": "0", "module": "C3", "scenario": "S0"}, {"value": "1.22E-12", "module": "C3", "scenario": "S1"}, {"value": "3.63E-13", "module": "C3", "scenario": "S2"}, {"value": "6.81E-14", "module": "C4", "scenario": "S0"}, {"value": "0", "module": "C4", "scenario": "S1"}, {"value": "0", "module": "C4", "scenario": "S2"}, {"value": "0", "module": "D", "scenario": "S0"}, {"value": "-2.13E-12", "module": "D", "scenario": "S1"}, {"value": "-5.6E-12", "module": "D", "scenario": "S2"}]}}, {"referenceToLCIAMethodDataSet": {"shortDescription": [{"value": "Versauerungspotenzial von Boden und Wasser (AP)", "lang": "de"}, {"value": "Acidification potential of land and water (AP)", "lang": "en"}], "type": "LCIA method data set", "refObjectId": "b5c611c6-def3-11e6-bf01-fe55135034f3", "uri": "../lciamethods/b5c611c6-def3-11e6-bf01-fe55135034f3.xml"}, "other": {"anies": [{"name": "referenceToUnitGroupDataSet", "value": {"shortDescription": [{"value": "mol H^(+)-Äq.", "lang": "de"}], "type": "unit group data set", "refObjectId": "42e089ac-92bf-4bf2-8ca1-5fc40d18f2ed", "uri": "../unitgroups/42e089ac-92bf-4bf2-8ca1-5fc40d18f2ed.xml"}}, {"value": "0.0061", "module": "A1-A3"}, {"value": "9.43E-05", "module": "A5"}, {"value": "3.14E-06", "module": "C1"}, {"value": "4.53E-06", "module": "C2"}, {"value": "0", "module": "C3", "scenario": "S0"}, {"value": "0.000119", "module": "C3", "scenario": "S1"}, {"value": "0.000234", "module": "C3", "scenario": "S2"}, {"value": "0.00014", "module": "C4", "scenario": "S0"}, {"value": "0", "module": "C4", "scenario": "S1"}, {"value": "0", "module": "C4", "scenario": "S2"}, {"value": "0", "module": "D", "scenario": "S0"}, {"value": "-0.000803", "module": "D", "scenario": "S1"}, {"value": "-0.00167", "module": "D", "scenario": "S2"}]}}, {"referenceToLCIAMethodDataSet": {"shortDescription": [{"value": "Eutrophierungspotenzial Süßwasser (EP-freshwater)", "lang": "de"}, {"value": "Eutrophication potential aquatic freshwater (EP-freshwater)", "lang": "en"}], "type": "LCIA method data set", "refObjectId": "b53ec18f-7377-4ad3-86eb-cc3f4f276b2b", "uri": "../lciamethods/b53ec18f-7377-4ad3-86eb-cc3f4f276b2b.xml"}, "other": {"anies": [{"name": "referenceToUnitGroupDataSet", "value": {"shortDescription": [{"value": "kg P-Äq.", "lang": "de"}], "type": "unit group data set", "refObjectId": "0429039d-a61d-4590-ba67-aa4a20a810a1", "uri": "../unitgroups/0429039d-a61d-4590-ba67-aa4a20a810a1.xml"}}, {"value": "1.36E-05", "module": "A1-A3"}, {"value": "1.96E-08", "module": "A5"}, {"value": "1.68E-09", "module": "C1"}, {"value": "1.03E-08", "module": "C2"}, {"value": "0", "module": "C3", "scenario": "S0"}, {"value": "2.36E-07", "module": "C3", "scenario": "S1"}, {"value": "2.01E-07", "module": "C3", "scenario": "S2"}, {"value": "8.21E-06", "module": "C4", "scenario": "S0"}, {"value": "0", "module": "C4", "scenario": "S1"}, {"value": "0", "module": "C4", "scenario": "S2"}, {"value": "0", "module": "D", "scenario": "S0"}, {"value": "-7.51E-07", "module": "D", "scenario": "S1"}, {"value": "-1.12E-06", "module": "D", "scenario": "S2"}]}}, {"referenceToLCIAMethodDataSet": {"shortDescription": [{"value": "Eutrophierungspotenzial Salzwasser (EP-marine)", "lang": "de"}, {"value": "Eutrophication potential aquatic marine (EP-marine)", "lang": "en"}], "type": "LCIA method data set", "refObjectId": "b5c619fa-def3-11e6-bf01-fe55135034f3", "uri": "../lciamethods/b5c619fa-def3-11e6-bf01-fe55135034f3.xml"}, "other": {"anies": [{"name": "referenceToUnitGroupDataSet", "value": {"shortDescription": [{"value": "kg N-Äq.", "lang": "de"}], "type": "unit group data set", "refObjectId": "d05bb823-ecdf-4686-8c40-bf1d9257859f", "uri": "../unitgroups/d05bb823-ecdf-4686-8c40-bf1d9257859f.xml"}}, {"value": "0.00164", "module": "A1-A3"}, {"value": "2.89E-05", "module": "A5"}, {"value": "1.48E-06", "module": "C1"}, {"value": "1.63E-06", "module": "C2"}, {"value": "0", "module": "C3", "scenario": "S0"}, {"value": "2.93E-05", "module": "C3", "scenario": "S1"}, {"value": "7.04E-05", "module": "C3", "scenario": "S2"}, {"value": "3.25E-05", "module": "C4", "scenario": "S0"}, {"value": "0", "module": "C4", "scenario": "S1"}, {"value": "0", "module": "C4", "scenario": "S2"}, {"value": "0", "module": "D", "scenario": "S0"}, {"value": "-0.000242", "module": "D", "scenario": "S1"}, {"value": "-0.000602", "module": "D", "scenario": "S2"}]}}, {"referenceToLCIAMethodDataSet": {"shortDescription": [{"value": "Eutrophierungspotenzial Land (EP-terrestrial)", "lang": "de"}, {"value": "Eutrophication potential terrestrial (EP-terrestrial)", "lang": "en"}], "type": "LCIA method data set", "refObjectId": "b5c614d2-def3-11e6-bf01-fe55135034f3", "uri": "../lciamethods/b5c614d2-def3-11e6-bf01-fe55135034f3.xml"}, "other": {"anies": [{"name": "referenceToUnitGroupDataSet", "value": {"shortDescription": [{"value": "mol N-Äq.", "lang": "de"}], "type": "unit group data set", "refObjectId": "71b4d617-0ec9-4d3f-b65e-e438940c2401", "uri": "../unitgroups/71b4d617-0ec9-4d3f-b65e-e438940c2401.xml"}}, {"value": "0.0183", "module": "A1-A3"}, {"value": "0.000444", "module": "A5"}, {"value": "1.65E-05", "module": "C1"}, {"value": "1.94E-05", "module": "C2"}, {"value": "0", "module": "C3", "scenario": "S0"}, {"value": "0.000345", "module": "C3", "scenario": "S1"}, {"value": "0.00113", "module": "C3", "scenario": "S2"}, {"value": "0.000357", "module": "C4", "scenario": "S0"}, {"value": "0", "module": "C4", "scenario": "S1"}, {"value": "0", "module": "C4", "scenario": "S2"}, {"value": "0", "module": "D", "scenario": "S0"}, {"value": "-0.00258", "module": "D", "scenario": "S1"}, {"value": "-0.00654", "module": "D", "scenario": "S2"}]}}, {"referenceToLCIAMethodDataSet": {"shortDescription": [{"value": "Bildungspotential für troposphärisches Ozon (POCP)", "lang": "de"}, {"value": "Formation potential of tropospheric ozone photochemical oxidants (POCP)", "lang": "en"}], "type": "LCIA method data set", "refObjectId": "b5c610fe-def3-11e6-bf01-fe55135034f3", "uri": "../lciamethods/b5c610fe-def3-11e6-bf01-fe55135034f3.xml"}, "other": {"anies": [{"name": "referenceToUnitGroupDataSet", "value": {"shortDescription": [{"value": "kg NMVOC-Äq.", "lang": "de"}], "type": "unit group data set", "refObjectId": "d27c25f8-fbc1-44c6-b47b-4adbae4199c6", "uri": "../unitgroups/d27c25f8-fbc1-44c6-b47b-4adbae4199c6.xml"}}, {"value": "0.00494", "module": "A1-A3"}, {"value": "7.68E-05", "module": "A5"}, {"value": "4.21E-06", "module": "C1"}, {"value": "4.55E-06", "module": "C2"}, {"value": "0", "module": "C3", "scenario": "S0"}, {"value": "7.83E-05", "module": "C3", "scenario": "S1"}, {"value": "0.000197", "module": "C3", "scenario": "S2"}, {"value": "0.000102", "module": "C4", "scenario": "S0"}, {"value": "0", "module": "C4", "scenario": "S1"}, {"value": "0", "module": "C4", "scenario": "S2"}, {"value": "0", "module": "D", "scenario": "S0"}, {"value": "-0.000982", "module": "D", "scenario": "S1"}, {"value": "-0.00174", "module": "D", "scenario": "S2"}]}}, {"referenceToLCIAMethodDataSet": {"shortDescription": [{"value": "Potenzial für den abiotischen Abbau nicht fossiler Ressourcen (ADPE)", "lang": "de"}, {"value": "Abiotic depletion potential for non fossil resources (ADPE)", "lang": "en"}], "type": "LCIA method data set", "refObjectId": "b2ad6494-c78d-11e6-9d9d-cec0c932ce01", "uri": "../lciamethods/b2ad6494-c78d-11e6-9d9d-cec0c932ce01.xml"}, "other": {"anies": [{"name": "referenceToUnitGroupDataSet", "value": {"shortDescription": [{"value": "kg Sb-Äq.", "lang": "de"}], "type": "unit group data set", "refObjectId": "54ccd2d9-a32a-4fc2-923d-f2c8c93e89d4", "uri": "../unitgroups/54ccd2d9-a32a-4fc2-923d-f2c8c93e89d4.xml"}}, {"value": "3.91E-06", "module": "A1-A3"}, {"value": "8.66E-10", "module": "A5"}, {"value": "1.05E-10", "module": "C1"}, {"value": "6.42E-10", "module": "C2"}, {"value": "0", "module": "C3", "scenario": "S0"}, {"value": "1.01E-08", "module": "C3", "scenario": "S1"}, {"value": "3.93E-09", "module": "C3", "scenario": "S2"}, {"value": "1.45E-09", "module": "C4", "scenario": "S0"}, {"value": "0", "module": "C4", "scenario": "S1"}, {"value": "0", "module": "C4", "scenario": "S2"}, {"value": "0", "module": "D", "scenario": "S0"}, {"value": "-4.48E-08", "module": "D", "scenario": "S1"}, {"value": "-5.81E-08", "module": "D", "scenario": "S2"}]}}, {"referenceToLCIAMethodDataSet": {"shortDescription": [{"value": "Potenzial für den abiotischen Abbau fossiler Brennstoffe (ADPF)", "lang": "de"}, {"value": "Abiotic depletion potential for fossil resources (ADPF)", "lang": "en"}], "type": "LCIA method data set", "refObjectId": "b2ad6110-c78d-11e6-9d9d-cec0c932ce01", "uri": "../lciamethods/b2ad6110-c78d-11e6-9d9d-cec0c932ce01.xml"}, "other": {"anies": [{"name": "referenceToUnitGroupDataSet", "value": {"shortDescription": [{"value": "MJ", "lang": "de"}], "type": "unit group data set", "refObjectId": "93a60a57-a3c8-11da-a746-0800200c9a66", "uri": "../unitgroups/93a60a57-a3c8-11da-a746-0800200c9a66.xml"}}, {"value": "43.3", "module": "A1-A3"}, {"value": "0.13", "module": "A5"}, {"value": "0.00809", "module": "C1"}, {"value": "0.0495", "module": "C2"}, {"value": "0", "module": "C3", "scenario": "S0"}, {"value": "1.14", "module": "C3", "scenario": "S1"}, {"value": "0.502", "module": "C3", "scenario": "S2"}, {"value": "0.343", "module": "C4", "scenario": "S0"}, {"value": "0", "module": "C4", "scenario": "S1"}, {"value": "0", "module": "C4", "scenario": "S2"}, {"value": "0", "module": "D", "scenario": "S0"}, {"value": "-17.5", "module": "D", "scenario": "S1"}, {"value": "-11.8", "module": "D", "scenario": "S2"}]}}, {"referenceToLCIAMethodDataSet": {"shortDescription": [{"value": "Wassernutzung (WDP)", "lang": "de"}, {"value": "Water use (WDP)", "lang": "en"}], "type": "LCIA method data set", "refObjectId": "b2ad66ce-c78d-11e6-9d9d-cec0c932ce01", "uri": "../lciamethods/b2ad66ce-c78d-11e6-9d9d-cec0c932ce01.xml"}, "other": {"anies": [{"name": "referenceToUnitGroupDataSet", "value": {"shortDescription": [{"value": "m^(3) Welt-Äq. entzogen", "lang": "de"}], "type": "unit group data set", "refObjectId": "6ae2df01-888e-46c8-b17d-49fa3869b476", "uri": "../unitgroups/6ae2df01-888e-46c8-b17d-49fa3869b476.xml"}}, {"value": "0.515", "module": "A1-A3"}, {"value": "0.052", "module": "A5"}, {"value": "4.41E-06", "module": "C1"}, {"value": "2.7E-05", "module": "C2"}, {"value": "0", "module": "C3", "scenario": "S0"}, {"value": "0.0303", "module": "C3", "scenario": "S1"}, {"value": "0.2", "module": "C3", "scenario": "S2"}, {"value": "0.00272", "module": "C4", "scenario": "S0"}, {"value": "0", "module": "C4", "scenario": "S1"}, {"value": "0", "module": "C4", "scenario": "S2"}, {"value": "0", "module": "D", "scenario": "S0"}, {"value": "-0.032", "module": "D", "scenario": "S1"}, {"value": "-0.0682", "module": "D", "scenario": "S2"}]}}, {"referenceToLCIAMethodDataSet": {"shortDescription": [{"value": "Auftreten von Krankheiten aufgrund von Feinstaubemissionen (PM)", "lang": "de"}, {"value": "Incidence of disease due to PM emissions (PM)", "lang": "en"}], "type": "LCIA method data set", "refObjectId": "b5c602c6-def3-11e6-bf01-fe55135034f3", "uri": "../lciamethods/b5c602c6-def3-11e6-bf01-fe55135034f3.xml"}, "other": {"anies": [{"name": "referenceToUnitGroupDataSet", "value": {"shortDescription": [{"value": "Krankheitsfälle", "lang": "de"}], "type": "unit group data set", "refObjectId": "3883559b-648f-4afc-8ba2-0bd24f3affa3", "uri": "../unitgroups/3883559b-648f-4afc-8ba2-0bd24f3affa3.xml"}}, {"value": "8.47E-08", "module": "A1-A3"}, {"value": "5.22E-10", "module": "A5"}, {"value": "3.74E-11", "module": "C1"}, {"value": "4.34E-11", "module": "C2"}, {"value": "0", "module": "C3", "scenario": "S0"}, {"value": "9.58E-10", "module": "C3", "scenario": "S1"}, {"value": "4.19E-09", "module": "C3", "scenario": "S2"}, {"value": "1.57E-09", "module": "C4", "scenario": "S0"}, {"value": "0", "module": "C4", "scenario": "S1"}, {"value": "0", "module": "C4", "scenario": "S2"}, {"value": "0", "module": "D", "scenario": "S0"}, {"value": "-6.82E-09", "module": "D", "scenario": "S1"}, {"value": "-1.09E-08", "module": "D", "scenario": "S2"}]}}, {"referenceToLCIAMethodDataSet": {"shortDescription": [{"value": "Wirkung durch Exposition des Menschen mit U235 (IR)", "lang": "de"}, {"value": "Human exposure efficiency relative to U235 (IR)", "lang": "en"}], "type": "LCIA method data set", "refObjectId": "b5c632be-def3-11e6-bf01-fe55135034f3", "uri": "../lciamethods/b5c632be-def3-11e6-bf01-fe55135034f3.xml"}, "other": {"anies": [{"name": "referenceToUnitGroupDataSet", "value": {"shortDescription": [{"value": "kBq U235-Äq.", "lang": "de"}], "type": "unit group data set", "refObjectId": "456b05bf-1415-44a9-9993-02452f554c09", "uri": "../unitgroups/456b05bf-1415-44a9-9993-02452f554c09.xml"}}, {"value": "0.0594", "module": "A1-A3"}, {"value": "0.000604", "module": "A5"}, {"value": "1.36E-06", "module": "C1"}, {"value": "8.32E-06", "module": "C2"}, {"value": "0", "module": "C3", "scenario": "S0"}, {"value": "0.0295", "module": "C3", "scenario": "S1"}, {"value": "0.00291", "module": "C3", "scenario": "S2"}, {"value": "0.000586", "module": "C4", "scenario": "S0"}, {"value": "0", "module": "C4", "scenario": "S1"}, {"value": "0", "module": "C4", "scenario": "S2"}, {"value": "0", "module": "D", "scenario": "S0"}, {"value": "-0.0262", "module": "D", "scenario": "S1"}, {"value": "-0.136", "module": "D", "scenario": "S2"}]}}, {"referenceToLCIAMethodDataSet": {"shortDescription": [{"value": "Toxizitätsvergleichseinheit für Ökosysteme (ETP-fw)", "lang": "de"}, {"value": "Comparative toxic unit for ecosystems (ETP-fw)", "lang": "en"}], "type": "LCIA method data set", "refObjectId": "ee1082d1-b0f7-43ca-a1f0-21e2a4a74511", "uri": "../lciamethods/ee1082d1-b0f7-43ca-a1f0-21e2a4a74511.xml"}, "other": {"anies": [{"name": "referenceToUnitGroupDataSet", "value": {"shortDescription": [{"value": "CTUe", "lang": "de"}], "type": "unit group data set", "refObjectId": "aa959ded-f1eb-4efb-9c5c-2d60be36b3e6", "uri": "../unitgroups/aa959ded-f1eb-4efb-9c5c-2d60be36b3e6.xml"}}, {"value": "23.6", "module": "A1-A3"}, {"value": "0.0614", "module": "A5"}, {"value": "0.00628", "module": "C1"}, {"value": "0.0384", "module": "C2"}, {"value": "0", "module": "C3", "scenario": "S0"}, {"value": "0.337", "module": "C3", "scenario": "S1"}, {"value": "0.234", "module": "C3", "scenario": "S2"}, {"value": "0.581", "module": "C4", "scenario": "S0"}, {"value": "0", "module": "C4", "scenario": "S1"}, {"value": "0", "module": "C4", "scenario": "S2"}, {"value": "0", "module": "D", "scenario": "S0"}, {"value": "-9.08", "module": "D", "scenario": "S1"}, {"value": "-6.39", "module": "D", "scenario": "S2"}]}}, {"referenceToLCIAMethodDataSet": {"shortDescription": [{"value": "Toxizitätsvergleichseinheit für Menschen (krebserregend) (HTP-c)", "lang": "de"}, {"value": "Comparative toxic unit for humans (carcinogenic) (HTP-c)", "lang": "en"}], "type": "LCIA method data set", "refObjectId": "2299222a-bbd8-474f-9d4f-4dd1f18aea7c", "uri": "../lciamethods/2299222a-bbd8-474f-9d4f-4dd1f18aea7c.xml"}, "other": {"anies": [{"name": "referenceToUnitGroupDataSet", "value": {"shortDescription": [{"value": "CTUh", "lang": "de"}], "type": "unit group data set", "refObjectId": "d4c9523e-2d7e-49fd-8469-998f547d3a70", "uri": "../unitgroups/d4c9523e-2d7e-49fd-8469-998f547d3a70.xml"}}, {"value": "1.41E-09", "module": "A1-A3"}, {"value": "3.75E-12", "module": "A5"}, {"value": "1.25E-13", "module": "C1"}, {"value": "7.66E-13", "module": "C2"}, {"value": "0", "module": "C3", "scenario": "S0"}, {"value": "1.93E-11", "module": "C3", "scenario": "S1"}, {"value": "1.57E-11", "module": "C3", "scenario": "S2"}, {"value": "9.14E-12", "module": "C4", "scenario": "S0"}, {"value": "0", "module": "C4", "scenario": "S1"}, {"value": "0", "module": "C4", "scenario": "S2"}, {"value": "0", "module": "D", "scenario": "S0"}, {"value": "-2.16E-10", "module": "D", "scenario": "S1"}, {"value": "-2.1E-10", "module": "D", "scenario": "S2"}]}}, {"referenceToLCIAMethodDataSet": {"shortDescription": [{"value": "Toxizitätsvergleichseinheit für Menschen (nicht krebserregend) (HTP-nc)", "lang": "de"}, {"value": "Comparative toxic unit for humans (noncarcinogenic) (HTP-nc)", "lang": "en"}], "type": "LCIA method data set", "refObjectId": "3af763a5-b7a1-48c9-9cee-1f223481fcef", "uri": "../lciamethods/3af763a5-b7a1-48c9-9cee-1f223481fcef.xml"}, "other": {"anies": [{"name": "referenceToUnitGroupDataSet", "value": {"shortDescription": [{"value": "CTUh", "lang": "de"}], "type": "unit group data set", "refObjectId": "d4c9523e-2d7e-49fd-8469-998f547d3a70", "uri": "../unitgroups/d4c9523e-2d7e-49fd-8469-998f547d3a70.xml"}}, {"value": "1.02E-07", "module": "A1-A3"}, {"value": "6.27E-11", "module": "A5"}, {"value": "5.28E-12", "module": "C1"}, {"value": "3.23E-11", "module": "C2"}, {"value": "0", "module": "C3", "scenario": "S0"}, {"value": "2.94E-10", "module": "C3", "scenario": "S1"}, {"value": "2.78E-10", "module": "C3", "scenario": "S2"}, {"value": "2.16E-10", "module": "C4", "scenario": "S0"}, {"value": "0", "module": "C4", "scenario": "S1"}, {"value": "0", "module": "C4", "scenario": "S2"}, {"value": "0", "module": "D", "scenario": "S0"}, {"value": "-7.85E-09", "module": "D", "scenario": "S1"}, {"value": "-4.1E-09", "module": "D", "scenario": "S2"}]}}, {"referenceToLCIAMethodDataSet": {"shortDescription": [{"value": "Bodenqualitätsindex (SQP)", "lang": "de"}, {"value": "Soil quality index (SQP)", "lang": "en"}], "type": "LCIA method data set", "refObjectId": "b2ad6890-c78d-11e6-9d9d-cec0c932ce01", "uri": "../lciamethods/b2ad6890-c78d-11e6-9d9d-cec0c932ce01.xml"}, "other": {"anies": [{"name": "referenceToUnitGroupDataSet", "value": {"shortDescription": [{"value": "SQP", "lang": "de"}], "type": "unit group data set", "refObjectId": "f130951c-e67f-4f7f-8dd4-665de3974e18", "uri": "../unitgroups/f130951c-e67f-4f7f-8dd4-665de3974e18.xml"}}, {"value": "86.8", "module": "A1-A3"}, {"value": "0.0505", "module": "A5"}, {"value": "0.00538", "module": "C1"}, {"value": "0.0329", "module": "C2"}, {"value": "0", "module": "C3", "scenario": "S0"}, {"value": "0.481", "module": "C3", "scenario": "S1"}, {"value": "0.222", "module": "C3", "scenario": "S2"}, {"value": "0.0699", "module": "C4", "scenario": "S0"}, {"value": "0", "module": "C4", "scenario": "S1"}, {"value": "0", "module": "C4", "scenario": "S2"}, {"value": "0", "module": "D", "scenario": "S0"}, {"value": "-0.781", "module": "D", "scenario": "S1"}, {"value": "-2.2", "module": "D", "scenario": "S2"}]}}]}, "otherAttributes": {"{http://www.indata.network/EPD/2019}epd-version": "1.2"}, "version": "1.1", "locations": "../ILCDLocations.xml"}