{"processInformation": {"dataSetInformation": {"UUID": "2812667f-8ca5-4ee1-a9ac-7ed13045b7ff", "name": {"baseName": [{"value": "Lava granulate", "lang": "en"}, {"value": "Lava Körnung", "lang": "de"}], "functionalUnitFlowProperties": [{"value": "granulate", "lang": "en"}]}, "classificationInformation": {"classification": [{"class": [{"value": "Mineralische Baustoffe", "level": 0, "classId": "1"}, {"value": "Zuschläge", "level": 1, "classId": "1.2"}, {"value": "Bims", "level": 2, "classId": "1.2.03"}], "name": "oekobau.dat"}]}, "generalComment": [{"value": "This data set has been modeled according to the European Standard EN 15804+A2 for Sustainable Building. Results are depicted in modules that allow the structured expression of results over the entire life cycle.", "lang": "en"}, {"value": "Dieser Datensatz wurde nach dem European Standard EN 15804+A2 für Nachhaltiges Bauen modelliert. Ergebnisse werden in Modulen abgebildet, die den strukturierten Ausdruck von Ergebnissen über den gesamten Lebenszyklus zulassen.", "lang": "de"}], "other": {"anies": [{"margins": 10, "description": [{"value": "Product system almost completely covered. Good technological, temporal and geographic representativeness.", "lang": "en"}, {"value": "Produktsystem weitgehend vollständig abgebildet. Gute technologische, zeitliche und geographische Repräsentativität.", "lang": "de"}]}]}}, "quantitativeReference": {"referenceToReferenceFlow": [100133], "type": "Reference flow(s)"}, "time": {"referenceYear": 2023, "dataSetValidUntil": 2026, "timeRepresentativenessDescription": [{"value": "Annual average", "lang": "en"}, {"value": "Jährlicher Durchschnitt", "lang": "de"}]}, "geography": {"locationOfOperationSupplyOrProduction": {"descriptionOfRestrictions": [{"value": "The data set represents the country specific situation in Germany, focusing on the main technologies, the region specific characteristics and / or import statistics.", "lang": "en"}, {"value": "Der Datensatz bildet die länderspezifische Situation in Deutschland ab. Dabei werden Haupttechnologien, spezifische regionale Charakteristiken und ggf. Importstatistiken berücksichtigt.", "lang": "de"}], "location": "DE"}}, "technology": {"technologyDescriptionAndIncludedProcesses": [{"value": "The LCA of lava granulate covers the process of the extraction of lava at open pit mine. Between the mine and processing, an average transport distance of 40 km is assumded. The system boundary of the finished product lava gravel is represented by the factory gate. Transports from the factory to the building site are not considered and must be included according to the system boundaries.", "lang": "en"}, {"value": "Die Lebenszyklusanalyse von Lava Körnung umfasst den Prozess der Lava-Gewinnung im Tagebau. Zwischen Tagebau und Aufbereitung wird eine mittlere Transportdistanz von 10 km angenommen. Die Systemgrenze bildet das fertige Produkt Lava-Kies am Werkstor. Transporte vom Werk zur Baustelle sind nicht berücksichtigt und müssen bei Systembetrachtungen eingerechnet werden.", "lang": "de"}], "technologicalApplicability": [{"value": "This product can be used in construction.", "lang": "en"}, {"value": "Dieses Produkt kann im Baubereich verwendet werden.", "lang": "de"}], "referenceToTechnologyFlowDiagrammOrPicture": [{"shortDescription": [{"value": "construction_de_lava granulate.jpg", "lang": "en"}], "type": "source data set", "refObjectId": "9853d17e-75e5-4bdc-a195-f69362444ac4", "version": "24.01.000", "uri": "../sources/9853d17e-75e5-4bdc-a195-f69362444ac4.xml"}]}}, "modellingAndValidation": {"LCIMethodAndAllocation": {"typeOfDataSet": "EPD", "other": {"anies": [{"name": "subType", "value": "generic dataset"}]}}, "dataSourcesTreatmentAndRepresentativeness": {"referenceToDataSource": [{"shortDescription": [{"value": "Ökologische Bilanzierung von Baustoffen und Gebäuden, 2000", "lang": "en"}], "type": "source data set", "refObjectId": "d2732220-5fbd-11db-b0de-0800200c9a66", "version": "24.01.000", "uri": "../sources/d2732220-5fbd-11db-b0de-0800200c9a66.xml"}, {"shortDescription": [{"value": "Baustoff-Ökobilanz. Wirkungsabschätzung und Auswertung in der Steine-Erden-Industrie, 1999", "lang": "en"}], "type": "source data set", "refObjectId": "8f4c8b35-1d8f-11dd-bd0b-0800200c9a66", "version": "24.01.000", "uri": "../sources/8f4c8b35-1d8f-11dd-bd0b-0800200c9a66.xml"}, {"shortDescription": [{"value": "Documentation of data quality management", "lang": "en"}], "type": "source data set", "refObjectId": "e3bd9bbf-2c3c-42aa-8892-fd13f1065ca5", "version": "24.01.000", "uri": "../sources/e3bd9bbf-2c3c-42aa-8892-fd13f1065ca5.xml"}, {"shortDescription": [{"value": "GaBi Database Edition 2021, CUP2021.01", "lang": "en"}], "type": "source data set", "refObjectId": "1cece811-7501-44d4-8067-9259bd5cb835", "version": "00.01.000", "uri": "../sources/1cece811-7501-44d4-8067-9259bd5cb835.xml"}, {"shortDescription": [{"value": "Sphera Managed LCA Content Databases (all versions)", "lang": "en"}], "type": "source data set", "refObjectId": "28d74cc0-db8b-4d7e-bc44-5f6d56ce0c4a", "version": "00.03.002", "uri": "../sources/28d74cc0-db8b-4d7e-bc44-5f6d56ce0c4a.xml"}], "useAdviceForDataSet": [{"value": "The data set represents a cradle to gate inventory. It can be used to characterise the supply chain situation of the respective commodity in a representative manner. Combination with individual unit processes using this commodity enables the generation of user-specific (product) LCAs.", "lang": "en"}, {"value": "Der Datensatz repräsentiert ein Cradle to Gate Inventar. Er kann verwendet werden, um die Lieferkette des jeweiligen Produktes in einer repräsentativen Weise zu charakterisieren. Die Kombination mit einzelnen Einheitenprozessen und diesem Produkt ermöglicht die Erstellung von anwenderspezifischen (Produkt-) LCAs.", "lang": "de"}]}, "validation": {"review": [{"referenceToNameOfReviewerAndInstitution": [{"shortDescription": [{"value": "Sphera Solutions GmbH", "lang": "en"}], "type": "contact data set", "refObjectId": "d7fa0337-f279-430d-becf-7f3111a85010", "version": "24.01.000", "uri": "../contacts/d7fa0337-f279-430d-becf-7f3111a85010.xml"}], "type": "Dependent internal review"}, {"referenceToNameOfReviewerAndInstitution": [{"shortDescription": [{"value": "Sphera Product Sustainability user forum", "lang": "en"}], "type": "contact data set", "refObjectId": "8f1306f0-7b83-4f36-a537-aa83f0498266", "version": "24.01.000", "uri": "../contacts/8f1306f0-7b83-4f36-a537-aa83f0498266.xml"}], "type": "Independent external review"}]}, "complianceDeclarations": {"compliance": [{"referenceToComplianceSystem": {"shortDescription": [{"value": "EN 15804+A2 (EF 3.1)", "lang": "de"}, {"value": "EN 15804+A2 (EF 3.1)", "lang": "en"}], "type": "source data set", "refObjectId": "d4aa3ec7-b1d7-4a4a-a6cb-37af88dcc902", "version": "00.01.000", "uri": "../sources/d4aa3ec7-b1d7-4a4a-a6cb-37af88dcc902.xml"}, "approvalOfOverallCompliance": "Fully compliant"}]}}, "administrativeInformation": {"dataGenerator": {"referenceToPersonOrEntityGeneratingTheDataSet": [{"shortDescription": [{"value": "Sphera Solutions GmbH", "lang": "en"}], "type": "contact data set", "refObjectId": "d7fa0337-f279-430d-becf-7f3111a85010", "version": "24.01.000", "uri": "../contacts/d7fa0337-f279-430d-becf-7f3111a85010.xml"}]}, "dataEntryBy": {"timeStamp": 1718121656000, "referenceToDataSetFormat": [{"shortDescription": [{"value": "ILCD format 1.1", "lang": "de"}, {"value": "ILCD format 1.1", "lang": "en"}], "type": "source data set", "refObjectId": "a97a0155-0234-4b87-b4ce-a45da52f2a40", "version": "01.00.000", "uri": "../sources/a97a0155-0234-4b87-b4ce-a45da52f2a40.xml"}, {"shortDescription": [{"value": "EPD-Datenformaterweiterungen v1.2", "lang": "de"}, {"value": "EPD Data Format Extensions v1.2", "lang": "en"}], "type": "source data set", "refObjectId": "a29449fd-aa2f-4de8-b5d7-4b06b43c6fde", "version": "00.01.000", "uri": "../sources/a29449fd-aa2f-4de8-b5d7-4b06b43c6fde.xml"}], "referenceToPersonOrEntityEnteringTheData": {"shortDescription": [{"value": "Sphera Solutions GmbH", "lang": "en"}], "type": "contact data set", "refObjectId": "d7fa0337-f279-430d-becf-7f3111a85010", "version": "24.01.000", "uri": "../contacts/d7fa0337-f279-430d-becf-7f3111a85010.xml"}}, "publicationAndOwnership": {"dataSetVersion": "20.24.070", "referenceToPrecedingDataSetVersion": [{"shortDescription": [{"value": "Lava granulate", "lang": "en"}], "type": "process data set", "refObjectId": "e2799f93-b221-48c5-b7ee-9dd39850e379", "uri": "https://www.oekobaudat.de/OEKOBAU.DAT/resource/processes/e2799f93-b221-48c5-b7ee-9dd39850e379?version=20.23.050"}], "referenceToRegistrationAuthority": {"shortDescription": [{"value": "Sphera Solutions GmbH", "lang": "en"}], "type": "contact data set", "refObjectId": "d7fa0337-f279-430d-becf-7f3111a85010", "version": "24.01.000", "uri": "../contacts/d7fa0337-f279-430d-becf-7f3111a85010.xml"}, "referenceToOwnershipOfDataSet": {"shortDescription": [{"value": "Sphera Solutions GmbH", "lang": "en"}], "type": "contact data set", "refObjectId": "d7fa0337-f279-430d-becf-7f3111a85010", "version": "24.01.000", "uri": "../contacts/d7fa0337-f279-430d-becf-7f3111a85010.xml"}, "copyright": true, "licenseType": "Free of charge for all users and uses", "accessRestrictions": [{"value": "The license conditions as stated on https://www.oekobaudat.de/apply.", "lang": "en"}, {"value": "Es gelten die Lizenzbedingungen wie sie auf https://www.oekobaudat.de/ genannt sind.", "lang": "de"}], "other": {"anies": [{"name": "referenceToPublisher", "value": {"shortDescription": [{"value": "BBSR", "lang": "en"}], "type": "contact data set", "refObjectId": "f11651e0-7877-11e3-981f-0800200c9a66", "version": "00.01.000", "uri": "../contacts/f11651e0-7877-11e3-981f-0800200c9a66.xml"}}]}}}, "exchanges": {"exchange": [{"dataSetInternalID": 100133, "referenceToFlowDataSet": {"shortDescription": [{"value": "Lava granulate", "lang": "en"}, {"value": "Lava Körnung", "lang": "de"}], "type": "flow data set", "refObjectId": "70b88044-1de7-4f9b-9406-1d61358ad410", "version": "24.01.000", "uri": "../flows/70b88044-1de7-4f9b-9406-1d61358ad410.xml"}, "meanAmount": 1.0, "referenceFlow": true, "resultingflowAmount": 1.0, "flowProperties": [{"name": [{"lang": "en", "value": "Mass"}, {"lang": "de", "value": "Masse"}], "uuid": "93a60a56-a3c8-11da-a746-0800200b9a66", "referenceFlowProperty": true, "meanValue": 1.0, "referenceUnit": "kg", "unitGroupUUID": "ad38d542-3fe9-439d-9b95-2f5f7752acaf"}], "materialProperties": [{"name": "gross density", "value": "1100.0", "unit": "kg/m^3", "unitDescription": "kilograms per cubic metre"}], "typeOfFlow": "Product flow", "classification": {"classHierarchy": "Valuable substances / Materials / Minerals", "name": "GaBiCategories"}}, {"dataSetInternalID": 100134, "referenceToFlowDataSet": {"shortDescription": [{"value": "Use of renewable primary energy as energy carrier (PERE)", "lang": "en"}, {"value": "Erneuerbare Primärenergie als Energieträger (PERE)", "lang": "de"}], "type": "flow data set", "refObjectId": "20f32be5-0398-4288-9b6d-accddd195317", "version": "24.01.000", "uri": "../flows/20f32be5-0398-4288-9b6d-accddd195317.xml"}, "exchange direction": "INPUT", "other": {"anies": [{"value": "0.00556096636735457", "module": "A1-A3"}, {"name": "referenceToUnitGroupDataSet", "value": {"shortDescription": [{"value": "MJ", "lang": "en"}], "type": "unit group data set", "refObjectId": "93a60a57-a3c8-11da-a746-0800200c9a66", "version": "03.00.000", "uri": "../unitgroups/93a60a57-a3c8-11da-a746-0800200c9a66.xml"}}]}, "resolvedFlowVersion": "38.00.000", "flowProperties": [], "typeOfFlow": "Other flow", "classification": {"classHierarchy": "Quantities", "name": "GaBiCategories"}}, {"dataSetInternalID": 100135, "referenceToFlowDataSet": {"shortDescription": [{"value": "Use of renewable primary energy resources used as raw materials (PERM)", "lang": "en"}, {"value": "Erneuerbare Primärenergie zur stofflichen Nutzung (PERM)", "lang": "de"}], "type": "flow data set", "refObjectId": "fb3ec0de-548d-4508-aea5-00b73bf6f702", "version": "24.01.000", "uri": "../flows/fb3ec0de-548d-4508-aea5-00b73bf6f702.xml"}, "exchange direction": "INPUT", "other": {"anies": [{"value": "0", "module": "A1-A3"}, {"name": "referenceToUnitGroupDataSet", "value": {"shortDescription": [{"value": "MJ", "lang": "en"}], "type": "unit group data set", "refObjectId": "93a60a57-a3c8-11da-a746-0800200c9a66", "version": "03.00.000", "uri": "../unitgroups/93a60a57-a3c8-11da-a746-0800200c9a66.xml"}}]}, "resolvedFlowVersion": "38.00.000", "flowProperties": [], "typeOfFlow": "Other flow", "classification": {"classHierarchy": "Quantities", "name": "GaBiCategories"}}, {"dataSetInternalID": 100136, "referenceToFlowDataSet": {"shortDescription": [{"value": "Total use of renewable primary energy (PERT)", "lang": "en"}, {"value": "Total erneuerbare Primärenergie (PERT)", "lang": "de"}], "type": "flow data set", "refObjectId": "53f97275-fa8a-4cdd-9024-65936002acd0", "version": "24.01.000", "uri": "../flows/53f97275-fa8a-4cdd-9024-65936002acd0.xml"}, "exchange direction": "INPUT", "other": {"anies": [{"value": "0.00556096636735457", "module": "A1-A3"}, {"name": "referenceToUnitGroupDataSet", "value": {"shortDescription": [{"value": "MJ", "lang": "en"}], "type": "unit group data set", "refObjectId": "93a60a57-a3c8-11da-a746-0800200c9a66", "version": "03.00.000", "uri": "../unitgroups/93a60a57-a3c8-11da-a746-0800200c9a66.xml"}}]}, "resolvedFlowVersion": "38.00.000", "flowProperties": [], "typeOfFlow": "Other flow", "classification": {"classHierarchy": "Quantities / Environmental quantities / EPD EN 15804 / LCI indicators", "name": "GaBiCategories"}}, {"dataSetInternalID": 100137, "referenceToFlowDataSet": {"shortDescription": [{"value": "Use of non renewable primary energy as energy carrier (PENRE)", "lang": "en"}, {"value": "Nicht-erneuerbare Primärenergie als Energieträger (PENRE)", "lang": "de"}], "type": "flow data set", "refObjectId": "ac857178-2b45-46ec-892a-a9a4332f0372", "version": "24.01.000", "uri": "../flows/ac857178-2b45-46ec-892a-a9a4332f0372.xml"}, "exchange direction": "INPUT", "other": {"anies": [{"value": "0.0512404830942577", "module": "A1-A3"}, {"name": "referenceToUnitGroupDataSet", "value": {"shortDescription": [{"value": "MJ", "lang": "en"}], "type": "unit group data set", "refObjectId": "93a60a57-a3c8-11da-a746-0800200c9a66", "version": "03.00.000", "uri": "../unitgroups/93a60a57-a3c8-11da-a746-0800200c9a66.xml"}}]}, "resolvedFlowVersion": "38.00.000", "flowProperties": [], "typeOfFlow": "Other flow", "classification": {"classHierarchy": "Quantities", "name": "GaBiCategories"}}, {"dataSetInternalID": 100138, "referenceToFlowDataSet": {"shortDescription": [{"value": "Use of non renewable primary energy resources used as raw materials (PENRM)", "lang": "en"}, {"value": "Nicht-erneuerbare Primärenergie zur stofflichen Nutzung (PENRM)", "lang": "de"}], "type": "flow data set", "refObjectId": "1421caa0-679d-4bf4-b282-0eb850ccae27", "version": "24.01.000", "uri": "../flows/1421caa0-679d-4bf4-b282-0eb850ccae27.xml"}, "exchange direction": "INPUT", "other": {"anies": [{"value": "0", "module": "A1-A3"}, {"name": "referenceToUnitGroupDataSet", "value": {"shortDescription": [{"value": "MJ", "lang": "en"}], "type": "unit group data set", "refObjectId": "93a60a57-a3c8-11da-a746-0800200c9a66", "version": "03.00.000", "uri": "../unitgroups/93a60a57-a3c8-11da-a746-0800200c9a66.xml"}}]}, "resolvedFlowVersion": "38.00.000", "flowProperties": [], "typeOfFlow": "Other flow", "classification": {"classHierarchy": "Quantities", "name": "GaBiCategories"}}, {"dataSetInternalID": 100139, "referenceToFlowDataSet": {"shortDescription": [{"value": "Total use of non renewable primary energy resource (PENRT)", "lang": "en"}, {"value": "Total nicht-erneuerbare Primärenergie (PENRT)", "lang": "de"}], "type": "flow data set", "refObjectId": "06159210-646b-4c8d-8583-da9b3b95a6c1", "version": "24.01.000", "uri": "../flows/06159210-646b-4c8d-8583-da9b3b95a6c1.xml"}, "exchange direction": "INPUT", "other": {"anies": [{"value": "0.0512404830942577", "module": "A1-A3"}, {"name": "referenceToUnitGroupDataSet", "value": {"shortDescription": [{"value": "MJ", "lang": "en"}], "type": "unit group data set", "refObjectId": "93a60a57-a3c8-11da-a746-0800200c9a66", "version": "03.00.000", "uri": "../unitgroups/93a60a57-a3c8-11da-a746-0800200c9a66.xml"}}]}, "resolvedFlowVersion": "38.00.000", "flowProperties": [], "typeOfFlow": "Other flow", "classification": {"classHierarchy": "Quantities / Environmental quantities / EPD EN 15804 / LCI indicators", "name": "GaBiCategories"}}, {"dataSetInternalID": 100140, "referenceToFlowDataSet": {"shortDescription": [{"value": "Use of secondary material (SM)", "lang": "en"}, {"value": "Einsatz von Sekundärstoffen (SM)", "lang": "de"}], "type": "flow data set", "refObjectId": "c6a1f35f-2d09-4f54-8dfb-97e502e1ce92", "version": "24.01.000", "uri": "../flows/c6a1f35f-2d09-4f54-8dfb-97e502e1ce92.xml"}, "exchange direction": "INPUT", "other": {"anies": [{"value": "0", "module": "A1-A3"}, {"name": "referenceToUnitGroupDataSet", "value": {"shortDescription": [{"value": "kg", "lang": "en"}], "type": "unit group data set", "refObjectId": "93a60a57-a4c8-11da-a746-0800200c9a66", "version": "03.00.000", "uri": "../unitgroups/93a60a57-a4c8-11da-a746-0800200c9a66.xml"}}]}, "resolvedFlowVersion": "38.00.000", "flowProperties": [], "typeOfFlow": "Other flow", "classification": {"classHierarchy": "Quantities / Environmental quantities / EPD EN 15804 / LCI indicators", "name": "GaBiCategories"}}, {"dataSetInternalID": 100141, "referenceToFlowDataSet": {"shortDescription": [{"value": "Use of renewable secondary fuels (SF)", "lang": "en"}, {"value": "Erneuerbare Sekundärbrennstoffe (SF)", "lang": "de"}], "type": "flow data set", "refObjectId": "64333088-a55f-4aa2-9a31-c10b07816787", "version": "24.01.000", "uri": "../flows/64333088-a55f-4aa2-9a31-c10b07816787.xml"}, "exchange direction": "INPUT", "other": {"anies": [{"value": "0", "module": "A1-A3"}, {"name": "referenceToUnitGroupDataSet", "value": {"shortDescription": [{"value": "MJ", "lang": "en"}], "type": "unit group data set", "refObjectId": "93a60a57-a3c8-11da-a746-0800200c9a66", "version": "03.00.000", "uri": "../unitgroups/93a60a57-a3c8-11da-a746-0800200c9a66.xml"}}]}, "resolvedFlowVersion": "38.00.000", "flowProperties": [], "typeOfFlow": "Other flow", "classification": {"classHierarchy": "Quantities / Environmental quantities / EPD EN 15804 / LCI indicators", "name": "GaBiCategories"}}, {"dataSetInternalID": 100142, "referenceToFlowDataSet": {"shortDescription": [{"value": "Use of non renewable secondary fuels (NRSF)", "lang": "en"}, {"value": "Nicht erneuerbare Sekundärbrennstoffe (NRSF)", "lang": "de"}], "type": "flow data set", "refObjectId": "89def144-d39a-4287-b86f-efde453ddcb2", "version": "24.01.000", "uri": "../flows/89def144-d39a-4287-b86f-efde453ddcb2.xml"}, "exchange direction": "INPUT", "other": {"anies": [{"value": "0", "module": "A1-A3"}, {"name": "referenceToUnitGroupDataSet", "value": {"shortDescription": [{"value": "MJ", "lang": "en"}], "type": "unit group data set", "refObjectId": "93a60a57-a3c8-11da-a746-0800200c9a66", "version": "03.00.000", "uri": "../unitgroups/93a60a57-a3c8-11da-a746-0800200c9a66.xml"}}]}, "resolvedFlowVersion": "38.00.000", "flowProperties": [], "typeOfFlow": "Other flow", "classification": {"classHierarchy": "Quantities / Environmental quantities / EPD EN 15804 / LCI indicators", "name": "GaBiCategories"}}, {"dataSetInternalID": 100143, "referenceToFlowDataSet": {"shortDescription": [{"value": "Net use of fresh water (FW)", "lang": "en"}, {"value": "Nettoeinsatz von Süßwasserressourcen (FW)", "lang": "de"}], "type": "flow data set", "refObjectId": "3cf952c8-f3a4-461d-8c96-96456ca62246", "version": "24.01.000", "uri": "../flows/3cf952c8-f3a4-461d-8c96-96456ca62246.xml"}, "exchange direction": "INPUT", "other": {"anies": [{"value": "5.28738513683552E-6", "module": "A1-A3"}, {"name": "referenceToUnitGroupDataSet", "value": {"shortDescription": [{"value": "m3", "lang": "en"}], "type": "unit group data set", "refObjectId": "93a60a57-a3c8-12da-a746-0800200c9a66", "version": "03.00.000", "uri": "../unitgroups/93a60a57-a3c8-12da-a746-0800200c9a66.xml"}}]}, "resolvedFlowVersion": "38.00.000", "flowProperties": [], "typeOfFlow": "Other flow", "classification": {"classHierarchy": "Quantities / Environmental quantities / EPD EN 15804 / LCI indicators", "name": "GaBiCategories"}}, {"dataSetInternalID": 100144, "referenceToFlowDataSet": {"shortDescription": [{"value": "Hazardous waste disposed (HWD)", "lang": "en"}, {"value": "Gefährlicher Abfall zur Deponie (HWD)", "lang": "de"}], "type": "flow data set", "refObjectId": "430f9e0f-59b2-46a0-8e0d-55e0e84948fc", "version": "24.01.000", "uri": "../flows/430f9e0f-59b2-46a0-8e0d-55e0e84948fc.xml"}, "exchange direction": "OUTPUT", "other": {"anies": [{"value": "2.18244947448794E-12", "module": "A1-A3"}, {"name": "referenceToUnitGroupDataSet", "value": {"shortDescription": [{"value": "kg", "lang": "en"}], "type": "unit group data set", "refObjectId": "93a60a57-a4c8-11da-a746-0800200c9a66", "version": "03.00.000", "uri": "../unitgroups/93a60a57-a4c8-11da-a746-0800200c9a66.xml"}}]}, "resolvedFlowVersion": "38.00.000", "flowProperties": [], "typeOfFlow": "Other flow", "classification": {"classHierarchy": "Quantities / Environmental quantities / EPD EN 15804 / LCI indicators", "name": "GaBiCategories"}}, {"dataSetInternalID": 100145, "referenceToFlowDataSet": {"shortDescription": [{"value": "Non harzardous waste disposed (NHWD)", "lang": "en"}, {"value": "Entsorgter nicht gefährlicher Abfall (NHWD)", "lang": "de"}], "type": "flow data set", "refObjectId": "b29ef66b-e286-4afa-949f-62f1a7b4d7fa", "version": "24.01.000", "uri": "../flows/b29ef66b-e286-4afa-949f-62f1a7b4d7fa.xml"}, "exchange direction": "OUTPUT", "other": {"anies": [{"value": "8.48470516444837E-6", "module": "A1-A3"}, {"name": "referenceToUnitGroupDataSet", "value": {"shortDescription": [{"value": "kg", "lang": "en"}], "type": "unit group data set", "refObjectId": "93a60a57-a4c8-11da-a746-0800200c9a66", "version": "03.00.000", "uri": "../unitgroups/93a60a57-a4c8-11da-a746-0800200c9a66.xml"}}]}, "resolvedFlowVersion": "38.00.000", "flowProperties": [], "typeOfFlow": "Other flow", "classification": {"classHierarchy": "Quantities / Environmental quantities / EPD EN 15804 / LCI indicators", "name": "GaBiCategories"}}, {"dataSetInternalID": 100146, "referenceToFlowDataSet": {"shortDescription": [{"value": "Radioactive waste disposed (RWD)", "lang": "en"}, {"value": "Entsorgter radioaktiver Abfall (RWD)", "lang": "de"}], "type": "flow data set", "refObjectId": "3449546e-52ad-4b39-b809-9fb77cea8ff6", "version": "24.01.000", "uri": "../flows/3449546e-52ad-4b39-b809-9fb77cea8ff6.xml"}, "exchange direction": "OUTPUT", "other": {"anies": [{"value": "6.91807669231907E-8", "module": "A1-A3"}, {"name": "referenceToUnitGroupDataSet", "value": {"shortDescription": [{"value": "kg", "lang": "en"}], "type": "unit group data set", "refObjectId": "93a60a57-a4c8-11da-a746-0800200c9a66", "version": "03.00.000", "uri": "../unitgroups/93a60a57-a4c8-11da-a746-0800200c9a66.xml"}}]}, "resolvedFlowVersion": "38.00.000", "flowProperties": [], "typeOfFlow": "Other flow", "classification": {"classHierarchy": "Quantities / Environmental quantities / EPD EN 15804 / LCI indicators", "name": "GaBiCategories"}}, {"dataSetInternalID": 100147, "referenceToFlowDataSet": {"shortDescription": [{"value": "Components for re-use (CRU)", "lang": "en"}, {"value": "Komponenten für die Wiederverwendung (CRU)", "lang": "de"}], "type": "flow data set", "refObjectId": "a2b32f97-3fc7-4af2-b209-525bc6426f33", "version": "24.01.000", "uri": "../flows/a2b32f97-3fc7-4af2-b209-525bc6426f33.xml"}, "exchange direction": "OUTPUT", "other": {"anies": [{"value": "0", "module": "A1-A3"}, {"name": "referenceToUnitGroupDataSet", "value": {"shortDescription": [{"value": "kg", "lang": "en"}], "type": "unit group data set", "refObjectId": "93a60a57-a4c8-11da-a746-0800200c9a66", "version": "03.00.000", "uri": "../unitgroups/93a60a57-a4c8-11da-a746-0800200c9a66.xml"}}]}, "resolvedFlowVersion": "38.00.000", "flowProperties": [], "typeOfFlow": "Other flow", "classification": {"classHierarchy": "Quantities / Environmental quantities / EPD EN 15804 / LCI indicators", "name": "GaBiCategories"}}, {"dataSetInternalID": 100148, "referenceToFlowDataSet": {"shortDescription": [{"value": "Materials for recycling  (MFR)", "lang": "en"}, {"value": "Stoffe zum Recycling (MFR)", "lang": "de"}], "type": "flow data set", "refObjectId": "d7fe48a5-4103-49c8-9aae-b0b5dfdbd6ae", "version": "24.01.000", "uri": "../flows/d7fe48a5-4103-49c8-9aae-b0b5dfdbd6ae.xml"}, "exchange direction": "OUTPUT", "other": {"anies": [{"value": "0", "module": "A1-A3"}, {"name": "referenceToUnitGroupDataSet", "value": {"shortDescription": [{"value": "kg", "lang": "en"}], "type": "unit group data set", "refObjectId": "93a60a57-a4c8-11da-a746-0800200c9a66", "version": "03.00.000", "uri": "../unitgroups/93a60a57-a4c8-11da-a746-0800200c9a66.xml"}}]}, "resolvedFlowVersion": "38.00.000", "flowProperties": [], "typeOfFlow": "Other flow", "classification": {"classHierarchy": "Quantities / Environmental quantities / EPD EN 15804 / LCI indicators", "name": "GaBiCategories"}}, {"dataSetInternalID": 100149, "referenceToFlowDataSet": {"shortDescription": [{"value": "Materials for energy recovery (MER)", "lang": "en"}, {"value": "Stoffe für die Energierückgewinnung (MER)", "lang": "de"}], "type": "flow data set", "refObjectId": "59a9181c-3aaf-46ee-8b13-2b3723b6e447", "version": "24.01.000", "uri": "../flows/59a9181c-3aaf-46ee-8b13-2b3723b6e447.xml"}, "exchange direction": "OUTPUT", "other": {"anies": [{"value": "0", "module": "A1-A3"}, {"name": "referenceToUnitGroupDataSet", "value": {"shortDescription": [{"value": "kg", "lang": "en"}], "type": "unit group data set", "refObjectId": "93a60a57-a4c8-11da-a746-0800200c9a66", "version": "03.00.000", "uri": "../unitgroups/93a60a57-a4c8-11da-a746-0800200c9a66.xml"}}]}, "resolvedFlowVersion": "38.00.000", "flowProperties": [], "typeOfFlow": "Other flow", "classification": {"classHierarchy": "Quantities / Environmental quantities / EPD EN 15804 / LCI indicators", "name": "GaBiCategories"}}, {"dataSetInternalID": 100150, "referenceToFlowDataSet": {"shortDescription": [{"value": "Exported electrical energy (EEE)", "lang": "en"}, {"value": "Exportierte elektrische Energie (EEE)", "lang": "de"}], "type": "flow data set", "refObjectId": "4da0c987-2b76-40d6-9e9e-82a017aaaf29", "version": "24.01.000", "uri": "../flows/4da0c987-2b76-40d6-9e9e-82a017aaaf29.xml"}, "exchange direction": "OUTPUT", "other": {"anies": [{"value": "0", "module": "A1-A3"}, {"name": "referenceToUnitGroupDataSet", "value": {"shortDescription": [{"value": "MJ", "lang": "en"}], "type": "unit group data set", "refObjectId": "93a60a57-a3c8-11da-a746-0800200c9a66", "version": "03.00.000", "uri": "../unitgroups/93a60a57-a3c8-11da-a746-0800200c9a66.xml"}}]}, "resolvedFlowVersion": "38.00.000", "flowProperties": [], "typeOfFlow": "Other flow", "classification": {"classHierarchy": "Quantities / Environmental quantities / EPD EN 15804 / LCI indicators", "name": "GaBiCategories"}}, {"dataSetInternalID": 100151, "referenceToFlowDataSet": {"shortDescription": [{"value": "Exported thermal energy (EET)", "lang": "en"}, {"value": "Exportierte thermische Energie (EET)", "lang": "de"}], "type": "flow data set", "refObjectId": "98daf38a-7a79-46d3-9a37-2b7bd0955810", "version": "24.01.000", "uri": "../flows/98daf38a-7a79-46d3-9a37-2b7bd0955810.xml"}, "exchange direction": "OUTPUT", "other": {"anies": [{"value": "0", "module": "A1-A3"}, {"name": "referenceToUnitGroupDataSet", "value": {"shortDescription": [{"value": "MJ", "lang": "en"}], "type": "unit group data set", "refObjectId": "93a60a57-a3c8-11da-a746-0800200c9a66", "version": "03.00.000", "uri": "../unitgroups/93a60a57-a3c8-11da-a746-0800200c9a66.xml"}}]}, "resolvedFlowVersion": "38.00.000", "flowProperties": [], "typeOfFlow": "Other flow", "classification": {"classHierarchy": "Quantities / Environmental quantities / EPD EN 15804 / LCI indicators", "name": "GaBiCategories"}}]}, "LCIAResults": {"LCIAResult": [{"referenceToLCIAMethodDataSet": {"shortDescription": [{"value": "Climate change", "lang": "en"}, {"value": "Globales Erwärmungspotenzial - total (GWP-total)", "lang": "de"}], "type": "LCIA method data set", "refObjectId": "a7ea142a-9749-11ed-a8fc-0242ac120002", "version": "24.01.000", "uri": "../lciamethods/a7ea142a-9749-11ed-a8fc-0242ac120002.xml"}, "other": {"anies": [{"value": "0.00402002564714602", "module": "A1-A3"}, {"name": "referenceToUnitGroupDataSet", "value": {"shortDescription": [{"value": "kg CO2 eq.", "lang": "en"}], "type": "unit group data set", "refObjectId": "1ebf3012-d0db-4de2-aefd-ef30cedb0be1", "version": "25.00.000", "uri": "../unitgroups/1ebf3012-d0db-4de2-aefd-ef30cedb0be1.xml"}}]}}, {"referenceToLCIAMethodDataSet": {"shortDescription": [{"value": "Climate change-Fossil", "lang": "en"}, {"value": "Globales Erwärmungspotenzial - fossil (GWP-fossil)", "lang": "de"}], "type": "LCIA method data set", "refObjectId": "a7ea19c0-9749-11ed-a8fc-0242ac120002", "version": "24.01.000", "uri": "../lciamethods/a7ea19c0-9749-11ed-a8fc-0242ac120002.xml"}, "other": {"anies": [{"value": "0.00404749384116432", "module": "A1-A3"}, {"name": "referenceToUnitGroupDataSet", "value": {"shortDescription": [{"value": "kg CO2 eq.", "lang": "en"}], "type": "unit group data set", "refObjectId": "1ebf3012-d0db-4de2-aefd-ef30cedb0be1", "version": "25.00.000", "uri": "../unitgroups/1ebf3012-d0db-4de2-aefd-ef30cedb0be1.xml"}}]}}, {"referenceToLCIAMethodDataSet": {"shortDescription": [{"value": "Climate change-Biogenic", "lang": "en"}, {"value": "Globales Erwärmungspotenzial - biogen (GWP-biogenic)", "lang": "de"}], "type": "LCIA method data set", "refObjectId": "a7ea186c-9749-11ed-a8fc-0242ac120002", "version": "24.01.000", "uri": "../lciamethods/a7ea186c-9749-11ed-a8fc-0242ac120002.xml"}, "other": {"anies": [{"value": "-0.000103079485325502", "module": "A1-A3"}, {"name": "referenceToUnitGroupDataSet", "value": {"shortDescription": [{"value": "kg CO2 eq.", "lang": "en"}], "type": "unit group data set", "refObjectId": "1ebf3012-d0db-4de2-aefd-ef30cedb0be1", "version": "25.00.000", "uri": "../unitgroups/1ebf3012-d0db-4de2-aefd-ef30cedb0be1.xml"}}]}}, {"referenceToLCIAMethodDataSet": {"shortDescription": [{"value": "Climate change-Land use and land use change", "lang": "en"}, {"value": "Globales Erwärmungspotenzial - luluc (GWP-luluc)", "lang": "de"}], "type": "LCIA method data set", "refObjectId": "a7ea1ae2-9749-11ed-a8fc-0242ac120002", "version": "24.01.000", "uri": "../lciamethods/a7ea1ae2-9749-11ed-a8fc-0242ac120002.xml"}, "other": {"anies": [{"value": "7.56112913072024E-5", "module": "A1-A3"}, {"name": "referenceToUnitGroupDataSet", "value": {"shortDescription": [{"value": "kg CO2 eq.", "lang": "en"}], "type": "unit group data set", "refObjectId": "1ebf3012-d0db-4de2-aefd-ef30cedb0be1", "version": "25.00.000", "uri": "../unitgroups/1ebf3012-d0db-4de2-aefd-ef30cedb0be1.xml"}}]}}, {"referenceToLCIAMethodDataSet": {"shortDescription": [{"value": "Depletion potenzial of the stratospheric ozone layer (ODP)", "lang": "en"}, {"value": "Abbaupotenzial der stratosphärischen Ozonschicht (ODP)", "lang": "de"}], "type": "LCIA method data set", "refObjectId": "b5c629d6-def3-11e6-bf01-fe55135034f3", "version": "24.01.000", "uri": "../lciamethods/b5c629d6-def3-11e6-bf01-fe55135034f3.xml"}, "other": {"anies": [{"value": "9.18496955255421E-16", "module": "A1-A3"}, {"name": "referenceToUnitGroupDataSet", "value": {"shortDescription": [{"value": "kg CFC-11 eq.", "lang": "en"}], "type": "unit group data set", "refObjectId": "d9e957c9-7309-4474-bf3a-7777df6c4e5b", "version": "25.00.000", "uri": "../unitgroups/d9e957c9-7309-4474-bf3a-7777df6c4e5b.xml"}}]}}, {"referenceToLCIAMethodDataSet": {"shortDescription": [{"value": "Acidifcation potential, Accumulated Exceedance (AP)", "lang": "en"}, {"value": "Versauerungspotenzial, kumulierte Überschreitung (AP)", "lang": "de"}], "type": "LCIA method data set", "refObjectId": "b5c611c6-def3-11e6-bf01-fe55135034f3", "version": "24.01.000", "uri": "../lciamethods/b5c611c6-def3-11e6-bf01-fe55135034f3.xml"}, "other": {"anies": [{"value": "2.20844047263197E-5", "module": "A1-A3"}, {"name": "referenceToUnitGroupDataSet", "value": {"shortDescription": [{"value": "Mole of H+ eq.", "lang": "en"}], "type": "unit group data set", "refObjectId": "42e089ac-92bf-4bf2-8ca1-5fc40d18f2ed", "version": "00.01.000", "uri": "../unitgroups/42e089ac-92bf-4bf2-8ca1-5fc40d18f2ed.xml"}}]}}, {"referenceToLCIAMethodDataSet": {"shortDescription": [{"value": "Eutrophication, freshwater", "lang": "en"}, {"value": "Eutrophierungspotenzial - Süßwasser (EP-freshwater)", "lang": "de"}], "type": "LCIA method data set", "refObjectId": "b53ec18f-7377-4ad3-86eb-cc3f4f276b2b", "version": "24.01.000", "uri": "../lciamethods/b53ec18f-7377-4ad3-86eb-cc3f4f276b2b.xml"}, "other": {"anies": [{"value": "1.06019337814917E-8", "module": "A1-A3"}, {"name": "referenceToUnitGroupDataSet", "value": {"shortDescription": [{"value": "kg P eq.", "lang": "en"}], "type": "unit group data set", "refObjectId": "0429039d-a61d-4590-ba67-aa4a20a810a1", "version": "25.00.000", "uri": "../unitgroups/0429039d-a61d-4590-ba67-aa4a20a810a1.xml"}}]}}, {"referenceToLCIAMethodDataSet": {"shortDescription": [{"value": "Eutrophication marine", "lang": "en"}, {"value": "Eutrophierungspotenzial - Salzwasser (EP-marine)", "lang": "de"}], "type": "LCIA method data set", "refObjectId": "b5c619fa-def3-11e6-bf01-fe55135034f3", "version": "24.01.000", "uri": "../lciamethods/b5c619fa-def3-11e6-bf01-fe55135034f3.xml"}, "other": {"anies": [{"value": "1.08289216000007E-5", "module": "A1-A3"}, {"name": "referenceToUnitGroupDataSet", "value": {"shortDescription": [{"value": "kg N eq.", "lang": "en"}], "type": "unit group data set", "refObjectId": "d05bb823-ecdf-4686-8c40-bf1d9257859f", "version": "00.00.003", "uri": "../unitgroups/d05bb823-ecdf-4686-8c40-bf1d9257859f.xml"}}]}}, {"referenceToLCIAMethodDataSet": {"shortDescription": [{"value": "Eutrophication, terrestrial", "lang": "en"}, {"value": "Eutrophierungspotenzial - Land (EP-terrestrial)", "lang": "de"}], "type": "LCIA method data set", "refObjectId": "b5c614d2-def3-11e6-bf01-fe55135034f3", "version": "24.01.000", "uri": "../lciamethods/b5c614d2-def3-11e6-bf01-fe55135034f3.xml"}, "other": {"anies": [{"value": "0.000120224667276815", "module": "A1-A3"}, {"name": "referenceToUnitGroupDataSet", "value": {"shortDescription": [{"value": "Mole of N eq.", "lang": "en"}], "type": "unit group data set", "refObjectId": "71b4d617-0ec9-4d3f-b65e-e438940c2401", "version": "00.00.003", "uri": "../unitgroups/71b4d617-0ec9-4d3f-b65e-e438940c2401.xml"}}]}}, {"referenceToLCIAMethodDataSet": {"shortDescription": [{"value": "Photochemical Ozone Creation Potential  (POCP)", "lang": "en"}, {"value": "Bildungspotenzial für troposphärisches Ozon (POCP)", "lang": "de"}], "type": "LCIA method data set", "refObjectId": "b5c610fe-def3-11e6-bf01-fe55135034f3", "version": "24.01.000", "uri": "../lciamethods/b5c610fe-def3-11e6-bf01-fe55135034f3.xml"}, "other": {"anies": [{"value": "2.92493704647004E-5", "module": "A1-A3"}, {"name": "referenceToUnitGroupDataSet", "value": {"shortDescription": [{"value": "kg NMVOC eq.", "lang": "en"}], "type": "unit group data set", "refObjectId": "d27c25f8-fbc1-44c6-b47b-4adbae4199c6", "version": "00.00.003", "uri": "../unitgroups/d27c25f8-fbc1-44c6-b47b-4adbae4199c6.xml"}}]}}, {"referenceToLCIAMethodDataSet": {"shortDescription": [{"value": "Resource use, minerals and metals", "lang": "en"}, {"value": "Potenzial für die Verknappung abiotischer Ressourcen  nicht fossile Ressourcen (ADPE)", "lang": "de"}], "type": "LCIA method data set", "refObjectId": "b2ad6494-c78d-11e6-9d9d-cec0c932ce01", "version": "24.01.000", "uri": "../lciamethods/b2ad6494-c78d-11e6-9d9d-cec0c932ce01.xml"}, "other": {"anies": [{"value": "6.65413786772746E-10", "module": "A1-A3"}, {"name": "referenceToUnitGroupDataSet", "value": {"shortDescription": [{"value": "kg Sb eq.", "lang": "en"}], "type": "unit group data set", "refObjectId": "54ccd2d9-a32a-4fc2-923d-f2c8c93e89d4", "version": "25.00.000", "uri": "../unitgroups/54ccd2d9-a32a-4fc2-923d-f2c8c93e89d4.xml"}}]}}, {"referenceToLCIAMethodDataSet": {"shortDescription": [{"value": "Resource use, fossils", "lang": "en"}, {"value": "Potenzial für die Verknappung abiotischer Ressourcen  fossile Brennstoffe (ADPF)", "lang": "de"}], "type": "LCIA method data set", "refObjectId": "b2ad6110-c78d-11e6-9d9d-cec0c932ce01", "version": "24.01.000", "uri": "../lciamethods/b2ad6110-c78d-11e6-9d9d-cec0c932ce01.xml"}, "other": {"anies": [{"value": "0.0512395957832125", "module": "A1-A3"}, {"name": "referenceToUnitGroupDataSet", "value": {"shortDescription": [{"value": "MJ", "lang": "en"}], "type": "unit group data set", "refObjectId": "93a60a57-a3c8-11da-a746-0800200c9a66", "version": "02.00.000", "uri": "../unitgroups/93a60a57-a3c8-11da-a746-0800200c9a66.xml"}}]}}, {"referenceToLCIAMethodDataSet": {"shortDescription": [{"value": "Water use", "lang": "en"}, {"value": "Wasser-Entzugspotenzial (Benutzer) (WDP)", "lang": "de"}], "type": "LCIA method data set", "refObjectId": "b2ad66ce-c78d-11e6-9d9d-cec0c932ce01", "version": "24.01.000", "uri": "../lciamethods/b2ad66ce-c78d-11e6-9d9d-cec0c932ce01.xml"}, "other": {"anies": [{"value": "2.77587875762481E-5", "module": "A1-A3"}, {"name": "referenceToUnitGroupDataSet", "value": {"shortDescription": [{"value": "m³ world equiv.", "lang": "en"}], "type": "unit group data set", "refObjectId": "6ae2df01-888e-46c8-b17d-49fa3869b476", "version": "00.00.003", "uri": "../unitgroups/6ae2df01-888e-46c8-b17d-49fa3869b476.xml"}}]}}]}, "otherAttributes": {"{http://www.indata.network/EPD/2019}epd-version": "1.2"}, "version": "1.1", "locations": "../ILCDLocations.xml"}