{"processInformation": {"dataSetInformation": {"UUID": "2cc49e5a-f0e0-4a1b-aa53-cf7caace7bbe", "name": {"baseName": [{"value": "Woven broadloom carpet, pile material solution-dyed polyamide 6.0 with a woven textile or a \"Silent Bac\" backing, both backings with recycled content,  maximum total pile weight 400 g/m²", "lang": "en"}, {"value": "Gewebter Teppichboden, Polmaterial spinngefärbtes Polyamid 6.0 mit einem gewebten Textilrücken oder \"Silent Bac\" Rückenausführung, beide Rückenausführungen mit Recyclingmaterial, maximales Poleinsatzgewicht 400 g/m²", "lang": "de"}], "functionalUnitFlowProperties": [{"lang": "en"}]}, "classificationInformation": {"classification": [{"class": [{"value": "Kunststoffe", "level": 0, "classId": "6"}, {"value": "Bodenbeläge", "level": 1, "classId": "6.2"}, {"value": "Textile Bodenbeläge", "level": 2, "classId": "6.2.05"}], "name": "OEKOBAU.DAT"}, {"class": [{"value": "02 Building products", "level": 0}, {"value": "Floor coverings", "level": 1}, {"value": "Floor coverings", "level": 2}], "name": "IBUCategories"}]}, "generalComment": [{"value": "Woven broadloom carpet having a pile material of solution-dyed polyamide 6 and a woven textile or a \"Silent Bac\" backing with recycled content. The maximum total pile weight is 400 g/m2.", "lang": "en"}, {"value": "Gewebter Teppichboden als Bahnenware mit einem Polmaterial aus spinngefärbtem Polyamid 6 und einem gewebten Textilrücken oder einem \"Silent Bac\"-Rücken mit Recyclingmaterial. Das maximale Poleinsatzgewicht beträgt 400 g/m².", "lang": "de"}], "other": {"anies": [{"scenario": [{"description": [{"value": "100% landfill disposal", "lang": "en"}, {"value": "Deponierung", "lang": "de"}], "name": "S1"}, {"description": [{"value": "100% municipal waste incineration", "lang": "en"}, {"value": "Müllverbrennung (Standard-Szenario)", "lang": "de"}], "name": "S2", "default": true}, {"description": [{"value": "100% recovery in the cement industry", "lang": "en"}, {"value": "Verwertung im Zementwerk", "lang": "de"}], "name": "S3"}]}]}}, "quantitativeReference": {"referenceToReferenceFlow": [0]}, "time": {"referenceYear": 2023, "dataSetValidUntil": 2028, "other": {"anies": [{"name": "publicationDateOfEPD", "value": 1690243200000}]}}, "geography": {"locationOfOperationSupplyOrProduction": {"location": "RER"}}, "technology": {"technologyDescriptionAndIncludedProcesses": [{"value": "Woven broadloom carpet having a pile material of polyamide 6 and a woven textile backing (COM 1000) or a felt backing (COM 1000 Silent Bac) made of polyester with recycled content.", "lang": "en"}, {"value": "Die Herstellungsprozesse sind: Weben, Aufbringen von Vorstrich und Rückenbeschichtung, Kantenschnitt, Verpacken \nTechnische Daten: \nProdukt Form: Bahnenware auf 4 m breiten Rollen\nArt der Herstellung: Gewebter Teppichboden\nFärbemethode: spinngefärbtes Garn\nGarntyp: Polyamid 6\nZweitrücken: Gewebter Textilrücken oder Vliesrücken aus recyceltem PET\nPoleinsatzgewicht:  max. 400 g/m²\nGesamtgewicht des Teppichs: max. 2100 g/m²  \nDeklarierte Einheit: \nDie angegebene Einheit bezieht sich auf 1 m²  produzierten textilen Bodenbelag. Der Output von Modul A5 \"Montage\" ist 1 m² verlegter textiler Bodenbelag. Die Rohdichte beträgt 540 g/m².", "lang": "de"}], "technologicalApplicability": [{"value": "According to the use class as defined in EN 1307 the products can be used in all professional areas with heavy use which require class 33 or less.", "lang": "en"}, {"value": "Gemäß der in /EN 1307/ definierten Gebrauchsklasse können die Produkte in allen professionellen Bereichen mit starker Beanspruchung eingesetzt werden, die die Klasse 33 oder weniger erfordern.", "lang": "de"}]}}, "modellingAndValidation": {"LCIMethodAndAllocation": {"typeOfDataSet": "EPD", "referenceToLCAMethodDetails": [{"shortDescription": [{"value": "Floor coverings.pdf", "lang": "en"}], "type": "source data set", "refObjectId": "85cd097a-a756-4efb-8ccd-db0257188ce4"}], "other": {"anies": [{"name": "subType", "value": "specific dataset"}]}}, "dataSourcesTreatmentAndRepresentativeness": {"referenceToDataSource": [{"shortDescription": [{"value": "GaBi Database (all versions)", "lang": "en"}], "type": "source data set", "refObjectId": "28d74cc0-db8b-4d7e-bc44-5f6d56ce0c4a"}, {"shortDescription": [{"value": "GaBi Database Edition 2022, CUP 2022.02", "lang": "en"}], "type": "source data set", "refObjectId": "94f442cb-662e-43ea-a792-4b0a35132e93"}], "useAdviceForDataSet": [{"value": "Scope: \nThe manufacturer declaration applies to the specific woven broadloom carpet with a woven textile or a \"Silent Bac\" backing and a total pile weight of 400 g/m2 .\nThe carpet is woven in the Fletco manufacturing site Bording, Denmark and it is precoated and back-coated in the Foamtex site, Bording, Denmark.\nThe declaration is only valid in conjunction with a valid GUT-PRODIS license of the product. \nSystem boundary: \nType of EPD:\nCradle-to-gate with options, modules C1-C4, module D, and additional modules A4, A5, B1, B2.\n\nSystem boundaries of modules A, B, C, D:\nModules C3, C4 and D are indicated separately for three end-of-life scenarios:\n\n1 - landfill disposal\n2 - municipal waste incineration\n3 - recovery in a cement plant\n\nA1-A3 Production:\nEnergy supply and production of the basic material, processing of secondary material, auxiliary material, transport of the material to the manufacturing site, emissions, waste water treatment, packaging material and waste processing up to the landfill disposal of residual waste (except radioactive waste). Benefits for generated electricity and steam due to the incineration of production waste are aggregated.\n\nA4 Transport:\nTransport of the packed textile floor covering from factory gate to the place of installation.\n\nA5 Installation:\nInstallation of the textile floor covering, processing of installation waste and packaging waste up to the landfill disposal of residual waste (except radioactive waste), the production of the amount of carpet that occurs as installation waste including its transport to the place of installation.\nGenerated electricity and steam due to the incineration of waste are listed in the result table as exported energy.\nPreparation of the floor and auxiliary materials (adhesives, fixing agents, PET connectors) are beyond the system boundaries and not taken into account.\n\nB1 Use:\nIndoor emissions during the use stage. After the first year, no product-related Volatile Organic Compound (VOC) emissions are relevant due to known VOC decay curves of the product.\n\nB2 Maintenance:\nCleaning of the textile floor covering for a period of 1 year:\nVacuum cleaning – electricity supply\nWet cleaning – electricity, water consumption, production of the cleaning agent, waste water treatment.\nThe declared values in this module have to be multiplied by the assumed service life of the floor covering in the building in question.\n\nB3 - B5:\nThe modules are not relevant within the assumed reference service life of 10 years.\n\nB6 - B7:\nNo energy and water input are required for the operation of the carpet in the use stage. The modules are not relevant and not declared.\n\nC1 De-construction:\nThe floor covering is de-constructed manually and no additional environmental impact is caused.\n\nC2 Transport:\nTransport of the carpet waste to a landfill, to the municipal waste incineration plant (MWI) or to the waste collection facility for recycling.\n\nC3 Waste processing:\nC3-1: Landfill disposal needs no waste processing.\nC3-2: Impact from waste incineration (plant with R1>0.6), generated electricity and steam are listed in the result table as exported energy.\nC3-3: Collection of the carpet waste for recovery in the cement industry, waste processing (granulating), transport to the cement plant, emissions from the incineration.\n\nC4 Disposal:\nC4-1: Impact from landfill disposal,\nC4-2: The carpet waste leaves the system in module C3-2,\nC4-3: The pre-processed carpet waste leaves the system in module C3-3.\n\nD Recycling potential:\nCalculated benefits result from materials exclusive secondary materials (net materials).\nD-A5: Benefits for generated energy due to incineration of packaging and installation waste (incineration plant with R1 > 0.6),\nD-1: Benefits for generated energy due to landfill disposal of carpet waste at the end of life,\nD-2: Benefits for generated energy due to incineration of carpet waste at the end-of-life (incineration plant with R1 > 0.6),\nD-3: Benefits for saved fossil energy and saved inorganic material due to recovery of the carpet in a cement plant.", "lang": "en"}, {"value": "Gültigkeitsbereich: \nDie Herstellererklärung gilt für den spezifischen gewebten Teppichboden mit einem gewebten Textil- oder \"Silent Bac\"-Rücken und einem Poleinsatzgewichtgewicht von 400 g/m².\nDer Teppich wird im Fletco-Werk Bording, Dänemark, gewebt und im Foamtex-Werk, Bording, Dänemark, beschichtet.\nDie Deklaration ist nur in Verbindung mit einer gültigen GUT-PRODIS-Lizenz für das Produkt gültig. \nSystemgrenze: \nTyp der EPD:\nWiege zum Werkstor mit Optionen, Modul C1-C4, Modul D und zusätzliche Module A4, A5, B1, B2.\nSystemgrenzen der Module A, B, C, D:\nDie Module C3, C4 und D sind separat für drei End-of-Life-Szenarien angegeben.", "lang": "de"}], "other": {"anies": [{"name": "referenceToOriginalEPD", "value": {"shortDescription": {"value": "Woven broadloom carpet, pile material solution-dyed polyamide 6.0 with a woven textile or a \"Silent Bac\" backing, both backings with recycled content,  maximum total pile weight 400 g/m².pdf", "defaultValue": "Woven broadloom carpet, pile material solution-dyed polyamide 6.0 with a woven textile or a \"Silent Bac\" backing, both backings with recycled content,  maximum total pile weight 400 g/m².pdf", "lstrings": [{"lang": "en", "value": "Woven broadloom carpet, pile material solution-dyed polyamide 6.0 with a woven textile or a \"Silent Bac\" backing, both backings with recycled content,  maximum total pile weight 400 g/m².pdf"}]}, "type": "source data set", "uuid": {"uuid": "3abab4dc-a142-4694-b348-761548c3aa7c"}, "refObjectId": "3abab4dc-a142-4694-b348-761548c3aa7c", "resourceURLs": ["https://oekobaudat.de/OEKOBAU.DAT/resource/sources/3abab4dc-a142-4694-b348-761548c3aa7c/Woven_broadloom_carpet_pile_material_solution-dyed_polyamide_6.0_with_a_woven_textile_or_a_Silent_Bac_backing_both_backings_with_recycled_content_maximum_total_pile_weight_400_gm_17129.pdf?version=00.01.000"]}}]}}, "validation": {"review": [{"referenceToNameOfReviewerAndInstitution": [{"shortDescription": [{"value": "Institut Bauen und Umwelt e. V.", "lang": "en"}], "type": "contact data set", "refObjectId": "d111dbec-b024-4be5-86c5-752d6eb2cf95", "uri": "../contacts/d111dbec-b024-4be5-86c5-752d6eb2cf95.xml"}], "type": "Accredited third party review"}]}, "complianceDeclarations": {"compliance": [{"referenceToComplianceSystem": {"shortDescription": [{"value": "DIN EN 15804+A2", "lang": "en"}], "type": "source data set", "refObjectId": "c0016b33-8cf7-415c-ac6e-deba0d21440d", "uri": "../sources/c0016b33-8cf7-415c-ac6e-deba0d21440d.xml"}}, {"referenceToComplianceSystem": {"shortDescription": [{"value": "ISO 14025", "lang": "en"}], "type": "source data set", "refObjectId": "4f2eb655-6e44-4874-a95a-e28f5442cd4d", "uri": "../sources/4f2eb655-6e44-4874-a95a-e28f5442cd4d.xml"}}]}}, "administrativeInformation": {"commissionerAndGoal": {"referenceToCommissioner": [{"shortDescription": [{"value": "Fletco Carpets A/S", "lang": "en"}], "type": "contact data set", "refObjectId": "3066f844-e2ce-406a-9d6a-86af6ef1f152", "uri": "../contacts/3066f844-e2ce-406a-9d6a-86af6ef1f152.xml"}]}, "dataGenerator": {"referenceToPersonOrEntityGeneratingTheDataSet": [{"shortDescription": [{"value": "Gemeinschaft umweltfreundlicher Teppichboden (GUT) e.V.", "lang": "en"}], "type": "contact data set", "refObjectId": "1e593d93-ef5b-4ddc-9b55-f58cf8960f3e", "uri": "../contacts/1e593d93-ef5b-4ddc-9b55-f58cf8960f3e.xml"}]}, "dataEntryBy": {"timeStamp": 1690243200000, "referenceToDataSetFormat": [{"shortDescription": [{"value": "ILCD Format", "lang": "en"}], "type": "source data set", "refObjectId": "a97a0155-0234-4b87-b4ce-a45da52f2a40", "uri": "../sources/a97a0155-0234-4b87-b4ce-a45da52f2a40.xml"}, {"shortDescription": [{"value": "EPD-Datenformaterweiterungen v1.2", "lang": "de"}, {"value": "EPD Data Format Extensions v1.2", "lang": "en"}], "type": "source data set", "refObjectId": "a29449fd-aa2f-4de8-b5d7-4b06b43c6fde", "uri": "../sources/a29449fd-aa2f-4de8-b5d7-4b06b43c6fde.xml"}]}, "publicationAndOwnership": {"dataSetVersion": "00.03.000", "referenceToRegistrationAuthority": {"shortDescription": [{"value": "Institut Bauen und Umwelt e. V.", "lang": "en"}], "type": "contact data set", "refObjectId": "d111dbec-b024-4be5-86c5-752d6eb2cf95", "uri": "../contacts/d111dbec-b024-4be5-86c5-752d6eb2cf95.xml"}, "registrationNumber": "EPD-FLE-20230274-CBC1-EN", "referenceToOwnershipOfDataSet": {"shortDescription": [{"value": "Fletco Carpets A/S", "lang": "en"}], "type": "contact data set", "refObjectId": "3066f844-e2ce-406a-9d6a-86af6ef1f152", "uri": "../contacts/3066f844-e2ce-406a-9d6a-86af6ef1f152.xml"}, "copyright": true, "licenseType": "Free of charge for all users and uses", "accessRestrictions": [{"value": "None", "lang": "en"}], "other": {"anies": [{"name": "referenceToPublisher", "value": {"shortDescription": [{"value": "Institut Bauen und Umwelt e. V.", "lang": "en"}], "type": "contact data set", "refObjectId": "d111dbec-b024-4be5-86c5-752d6eb2cf95", "uri": "../contacts/d111dbec-b024-4be5-86c5-752d6eb2cf95.xml"}}]}}}, "exchanges": {"exchange": [{"dataSetInternalID": 0, "referenceToFlowDataSet": {"shortDescription": [{"value": "Woven broadloom carpet, pile material solution-dyed polyamide 6.0 with a woven textile or a \"Silent Bac\" backing, both backings with recycled content,  maximum total pile weight 400 g/m² (Gewebter Teppichboden, Polmaterial 400 g/m² spinngefärbtes Polyamid 6.0 mit einem gewebten Textilrücken oder \"Silent Bac\" Rückenausführung)", "lang": "en"}], "type": "flow data set", "refObjectId": "aa13714f-7930-bdcd-2bef-24b268285c48", "uri": "../flows/aa13714f-7930-bdcd-2bef-24b268285c48.xml"}, "meanAmount": 1.0, "referencesToDataSource": {}, "referenceFlow": true, "resolvedFlowVersion": "00.03.000", "resultingflowAmount": 1.0, "flowProperties": [{"name": [{"lang": "en", "value": "Area"}, {"lang": "de", "value": "Fläche"}], "uuid": "93a60a56-a3c8-19da-a746-0800200c9a66", "referenceFlowProperty": true, "meanValue": 1.0, "referenceUnit": "qm", "unitGroupUUID": "c20a03d7-bd90-4569-bc94-66cfd364dfc8"}], "materialProperties": [{"name": "layer thickness", "value": "0.004", "unit": "m", "unitDescription": "meters"}, {"name": "grammage", "value": "2.144", "unit": "kg/m^2", "unitDescription": "kilograms per square meter"}, {"name": "gross density", "value": "540.0", "unit": "kg/m^3", "unitDescription": "kilograms per cubic metre"}], "typeOfFlow": "Product flow", "classification": {"classHierarchy": "Kunststoffe / Bodenbeläge / Textile Bodenbeläge", "name": "OEKOBAU.DAT"}}, {"dataSetInternalID": 1, "referenceToFlowDataSet": {"shortDescription": [{"value": "Renewable primary energy as energy carrier (PERE)", "lang": "en"}, {"value": "Erneuerbare Primärenergie als Energieträger (PERE)", "lang": "de"}], "type": "flow data set", "refObjectId": "20f32be5-0398-4288-9b6d-accddd195317", "uri": "../flows/20f32be5-0398-4288-9b6d-accddd195317.xml"}, "exchange direction": "INPUT", "other": {"anies": [{"name": "referenceToUnitGroupDataSet", "value": {"shortDescription": [{"value": "MJ", "lang": "en"}], "type": "unit group data set", "refObjectId": "93a60a57-a3c8-11da-a746-0800200c9a66", "uri": "../unitgroups/93a60a57-a3c8-11da-a746-0800200c9a66.xml"}}, {"value": "26.93", "module": "A1-A3"}, {"value": "0.09817", "module": "A4"}, {"value": "2.45753", "module": "A5"}, {"value": "0", "module": "B1"}, {"value": "3.685", "module": "B2"}, {"value": "0", "module": "C1"}, {"value": "0.005513", "module": "C2"}, {"value": "0.2369", "module": "C3", "scenario": "S2"}, {"value": "0.3613", "module": "C3", "scenario": "S3"}, {"value": "0.1773", "module": "C4"}, {"value": "-0.5499", "module": "D", "scenario": "S0"}, {"value": "0", "module": "D", "scenario": "S1"}, {"value": "-3.211", "module": "D", "scenario": "S2"}, {"value": "-0.2846", "module": "D", "scenario": "S3"}]}, "resolvedFlowVersion": "38.00.000", "flowProperties": [], "typeOfFlow": "Other flow", "classification": {"classHierarchy": "Quantities", "name": "GaBiCategories"}}, {"dataSetInternalID": 2, "referenceToFlowDataSet": {"shortDescription": [{"value": "Renewable primary energy resources as material utilization (PERM)", "lang": "en"}, {"value": "Erneuerbare Primärenergie zur stofflichen Nutzung (PERM)", "lang": "de"}], "type": "flow data set", "refObjectId": "fb3ec0de-548d-4508-aea5-00b73bf6f702", "uri": "../flows/fb3ec0de-548d-4508-aea5-00b73bf6f702.xml"}, "exchange direction": "INPUT", "other": {"anies": [{"name": "referenceToUnitGroupDataSet", "value": {"shortDescription": [{"value": "MJ", "lang": "en"}], "type": "unit group data set", "refObjectId": "93a60a57-a3c8-11da-a746-0800200c9a66", "uri": "../unitgroups/93a60a57-a3c8-11da-a746-0800200c9a66.xml"}}, {"value": "0", "module": "A1-A3"}, {"value": "0", "module": "A4"}, {"value": "0", "module": "A5"}, {"value": "0", "module": "B1"}, {"value": "0", "module": "B2"}, {"value": "0", "module": "C1"}, {"value": "0", "module": "C2"}, {"value": "0", "module": "C3", "scenario": "S2"}, {"value": "0", "module": "C3", "scenario": "S3"}, {"value": "0", "module": "C4"}, {"value": "0", "module": "D", "scenario": "S0"}, {"value": "0", "module": "D", "scenario": "S1"}, {"value": "0", "module": "D", "scenario": "S2"}, {"value": "0", "module": "D", "scenario": "S3"}]}, "resolvedFlowVersion": "38.00.000", "flowProperties": [], "typeOfFlow": "Other flow", "classification": {"classHierarchy": "Quantities", "name": "GaBiCategories"}}, {"dataSetInternalID": 3, "referenceToFlowDataSet": {"shortDescription": [{"value": "Total use of renewable primary energy resources (PERT)", "lang": "en"}, {"value": "Total erneuerbare Primärenergie (PERT)", "lang": "de"}], "type": "flow data set", "refObjectId": "53f97275-fa8a-4cdd-9024-65936002acd0", "uri": "../flows/53f97275-fa8a-4cdd-9024-65936002acd0.xml"}, "exchange direction": "INPUT", "other": {"anies": [{"name": "referenceToUnitGroupDataSet", "value": {"shortDescription": [{"value": "MJ", "lang": "en"}], "type": "unit group data set", "refObjectId": "93a60a57-a3c8-11da-a746-0800200c9a66", "uri": "../unitgroups/93a60a57-a3c8-11da-a746-0800200c9a66.xml"}}, {"value": "26.93", "module": "A1-A3"}, {"value": "0.09817", "module": "A4"}, {"value": "2.45753", "module": "A5"}, {"value": "0", "module": "B1"}, {"value": "3.685", "module": "B2"}, {"value": "0", "module": "C1"}, {"value": "0.005513", "module": "C2"}, {"value": "0.2369", "module": "C3", "scenario": "S2"}, {"value": "0.3613", "module": "C3", "scenario": "S3"}, {"value": "0.1773", "module": "C4"}, {"value": "-0.5499", "module": "D", "scenario": "S0"}, {"value": "0", "module": "D", "scenario": "S1"}, {"value": "-3.211", "module": "D", "scenario": "S2"}, {"value": "-0.2846", "module": "D", "scenario": "S3"}]}, "resolvedFlowVersion": "38.00.000", "flowProperties": [], "typeOfFlow": "Other flow", "classification": {"classHierarchy": "Quantities / Environmental quantities / EPD EN 15804 / LCI indicators", "name": "GaBiCategories"}}, {"dataSetInternalID": 4, "referenceToFlowDataSet": {"shortDescription": [{"value": "Non renewable primary energy as energy carrier (PENRE)", "lang": "en"}, {"value": "Nicht-erneuerbare Primärenergie als Energieträger (PENRE)", "lang": "de"}], "type": "flow data set", "refObjectId": "ac857178-2b45-46ec-892a-a9a4332f0372", "uri": "../flows/ac857178-2b45-46ec-892a-a9a4332f0372.xml"}, "exchange direction": "INPUT", "other": {"anies": [{"name": "referenceToUnitGroupDataSet", "value": {"shortDescription": [{"value": "MJ", "lang": "en"}], "type": "unit group data set", "refObjectId": "93a60a57-a3c8-11da-a746-0800200c9a66", "uri": "../unitgroups/93a60a57-a3c8-11da-a746-0800200c9a66.xml"}}, {"value": "128.3", "module": "A1-A3"}, {"value": "1.731", "module": "A4"}, {"value": "16.1952", "module": "A5"}, {"value": "0", "module": "B1"}, {"value": "5.898", "module": "B2"}, {"value": "0", "module": "C1"}, {"value": "0.09721", "module": "C2"}, {"value": "30.554", "module": "C3", "scenario": "S2"}, {"value": "30.996", "module": "C3", "scenario": "S3"}, {"value": "2.157", "module": "C4"}, {"value": "-2.01", "module": "D", "scenario": "S0"}, {"value": "0", "module": "D", "scenario": "S1"}, {"value": "-11.83", "module": "D", "scenario": "S2"}, {"value": "-26.44", "module": "D", "scenario": "S3"}]}, "resolvedFlowVersion": "38.00.000", "flowProperties": [], "typeOfFlow": "Other flow", "classification": {"classHierarchy": "Quantities", "name": "GaBiCategories"}}, {"dataSetInternalID": 5, "referenceToFlowDataSet": {"shortDescription": [{"value": "Non renewable primary energy as material utilization (PENRM)", "lang": "en"}, {"value": "Nicht-erneuerbare Primärenergie zur stofflichen Nutzung (PENRM)", "lang": "de"}], "type": "flow data set", "refObjectId": "1421caa0-679d-4bf4-b282-0eb850ccae27", "uri": "../flows/1421caa0-679d-4bf4-b282-0eb850ccae27.xml"}, "exchange direction": "INPUT", "other": {"anies": [{"name": "referenceToUnitGroupDataSet", "value": {"shortDescription": [{"value": "MJ", "lang": "en"}], "type": "unit group data set", "refObjectId": "93a60a57-a3c8-11da-a746-0800200c9a66", "uri": "../unitgroups/93a60a57-a3c8-11da-a746-0800200c9a66.xml"}}, {"value": "30.8", "module": "A1-A3"}, {"value": "0", "module": "A4"}, {"value": "-1.579", "module": "A5"}, {"value": "0", "module": "B1"}, {"value": "0", "module": "B2"}, {"value": "0", "module": "C1"}, {"value": "0", "module": "C2"}, {"value": "-29.221", "module": "C3", "scenario": "S2"}, {"value": "-29.221", "module": "C3", "scenario": "S3"}, {"value": "0", "module": "C4"}, {"value": "0", "module": "D", "scenario": "S0"}, {"value": "0", "module": "D", "scenario": "S1"}, {"value": "0", "module": "D", "scenario": "S2"}, {"value": "0", "module": "D", "scenario": "S3"}]}, "resolvedFlowVersion": "38.00.000", "flowProperties": [], "typeOfFlow": "Other flow", "classification": {"classHierarchy": "Quantities", "name": "GaBiCategories"}}, {"dataSetInternalID": 6, "referenceToFlowDataSet": {"shortDescription": [{"value": "Total use of non renewable primary energy resources (PENRT)", "lang": "en"}, {"value": "Total nicht erneuerbare Primärenergie (PENRT)", "lang": "de"}], "type": "flow data set", "refObjectId": "06159210-646b-4c8d-8583-da9b3b95a6c1", "uri": "../flows/06159210-646b-4c8d-8583-da9b3b95a6c1.xml"}, "exchange direction": "INPUT", "other": {"anies": [{"name": "referenceToUnitGroupDataSet", "value": {"shortDescription": [{"value": "MJ", "lang": "en"}], "type": "unit group data set", "refObjectId": "93a60a57-a3c8-11da-a746-0800200c9a66", "uri": "../unitgroups/93a60a57-a3c8-11da-a746-0800200c9a66.xml"}}, {"value": "159.1", "module": "A1-A3"}, {"value": "1.731", "module": "A4"}, {"value": "14.6162", "module": "A5"}, {"value": "0", "module": "B1"}, {"value": "5.898", "module": "B2"}, {"value": "0", "module": "C1"}, {"value": "0.09721", "module": "C2"}, {"value": "1.333", "module": "C3", "scenario": "S2"}, {"value": "1.775", "module": "C3", "scenario": "S3"}, {"value": "2.157", "module": "C4"}, {"value": "-2.01", "module": "D", "scenario": "S0"}, {"value": "0", "module": "D", "scenario": "S1"}, {"value": "-11.83", "module": "D", "scenario": "S2"}, {"value": "-26.44", "module": "D", "scenario": "S3"}]}, "resolvedFlowVersion": "38.00.000", "flowProperties": [], "typeOfFlow": "Other flow", "classification": {"classHierarchy": "Quantities / Environmental quantities / EPD EN 15804 / LCI indicators", "name": "GaBiCategories"}}, {"dataSetInternalID": 7, "referenceToFlowDataSet": {"shortDescription": [{"value": "Use of secondary material (SM)", "lang": "en"}, {"value": "Einsatz von Sekundärstoffen (SM)", "lang": "de"}], "type": "flow data set", "refObjectId": "c6a1f35f-2d09-4f54-8dfb-97e502e1ce92", "uri": "../flows/c6a1f35f-2d09-4f54-8dfb-97e502e1ce92.xml"}, "exchange direction": "INPUT", "other": {"anies": [{"name": "referenceToUnitGroupDataSet", "value": {"shortDescription": [{"value": "kg", "lang": "en"}], "type": "unit group data set", "refObjectId": "ad38d542-3fe9-439d-9b95-2f5f7752acaf", "uri": "../unitgroups/ad38d542-3fe9-439d-9b95-2f5f7752acaf.xml"}}, {"value": "0.52", "module": "A1-A3"}, {"value": "0", "module": "A4"}, {"value": "0.0468", "module": "A5"}, {"value": "0", "module": "B1"}, {"value": "0", "module": "B2"}, {"value": "0", "module": "C1"}, {"value": "0", "module": "C2"}, {"value": "0", "module": "C3", "scenario": "S2"}, {"value": "0", "module": "C3", "scenario": "S3"}, {"value": "0", "module": "C4"}, {"value": "0", "module": "D", "scenario": "S0"}, {"value": "0", "module": "D", "scenario": "S1"}, {"value": "0", "module": "D", "scenario": "S2"}, {"value": "0.34", "module": "D", "scenario": "S3"}]}, "resolvedFlowVersion": "38.00.000", "flowProperties": [], "typeOfFlow": "Other flow", "classification": {"classHierarchy": "Quantities / Environmental quantities / EPD EN 15804 / LCI indicators", "name": "GaBiCategories"}}, {"dataSetInternalID": 8, "referenceToFlowDataSet": {"shortDescription": [{"value": "Use of renewable secondary fuels (RSF)", "lang": "en"}, {"value": "Erneuerbare Sekundärbrennstoffe (RSF)", "lang": "de"}], "type": "flow data set", "refObjectId": "64333088-a55f-4aa2-9a31-c10b07816787", "uri": "../flows/64333088-a55f-4aa2-9a31-c10b07816787.xml"}, "exchange direction": "INPUT", "other": {"anies": [{"name": "referenceToUnitGroupDataSet", "value": {"shortDescription": [{"value": "MJ", "lang": "en"}], "type": "unit group data set", "refObjectId": "93a60a57-a3c8-11da-a746-0800200c9a66", "uri": "../unitgroups/93a60a57-a3c8-11da-a746-0800200c9a66.xml"}}, {"value": "0", "module": "A1-A3"}, {"value": "0", "module": "A4"}, {"value": "0", "module": "A5"}, {"value": "0", "module": "B1"}, {"value": "0", "module": "B2"}, {"value": "0", "module": "C1"}, {"value": "0", "module": "C2"}, {"value": "0", "module": "C3", "scenario": "S2"}, {"value": "0", "module": "C3", "scenario": "S3"}, {"value": "0", "module": "C4"}, {"value": "0", "module": "D", "scenario": "S0"}, {"value": "0", "module": "D", "scenario": "S1"}, {"value": "0", "module": "D", "scenario": "S2"}, {"value": "0", "module": "D", "scenario": "S3"}]}, "resolvedFlowVersion": "38.00.000", "flowProperties": [], "typeOfFlow": "Other flow", "classification": {"classHierarchy": "Quantities / Environmental quantities / EPD EN 15804 / LCI indicators", "name": "GaBiCategories"}}, {"dataSetInternalID": 9, "referenceToFlowDataSet": {"shortDescription": [{"value": "Use of non renewable secondary fuels (NRSF)", "lang": "en"}, {"value": "Nicht erneuerbare Sekundärbrennstoffe (NRSF)", "lang": "de"}], "type": "flow data set", "refObjectId": "89def144-d39a-4287-b86f-efde453ddcb2", "uri": "../flows/89def144-d39a-4287-b86f-efde453ddcb2.xml"}, "exchange direction": "INPUT", "other": {"anies": [{"name": "referenceToUnitGroupDataSet", "value": {"shortDescription": [{"value": "MJ", "lang": "en"}], "type": "unit group data set", "refObjectId": "93a60a57-a3c8-11da-a746-0800200c9a66", "uri": "../unitgroups/93a60a57-a3c8-11da-a746-0800200c9a66.xml"}}, {"value": "0", "module": "A1-A3"}, {"value": "0", "module": "A4"}, {"value": "0", "module": "A5"}, {"value": "0", "module": "B1"}, {"value": "0", "module": "B2"}, {"value": "0", "module": "C1"}, {"value": "0", "module": "C2"}, {"value": "0", "module": "C3", "scenario": "S2"}, {"value": "0", "module": "C3", "scenario": "S3"}, {"value": "0", "module": "C4"}, {"value": "0", "module": "D", "scenario": "S0"}, {"value": "0", "module": "D", "scenario": "S1"}, {"value": "0", "module": "D", "scenario": "S2"}, {"value": "0", "module": "D", "scenario": "S3"}]}, "resolvedFlowVersion": "38.00.000", "flowProperties": [], "typeOfFlow": "Other flow", "classification": {"classHierarchy": "Quantities / Environmental quantities / EPD EN 15804 / LCI indicators", "name": "GaBiCategories"}}, {"dataSetInternalID": 10, "referenceToFlowDataSet": {"shortDescription": [{"value": "Use of net fresh water (FW)", "lang": "en"}, {"value": "Einsatz von Süßwasserressourcen (FW)", "lang": "de"}], "type": "flow data set", "refObjectId": "3cf952c8-f3a4-461d-8c96-96456ca62246", "uri": "../flows/3cf952c8-f3a4-461d-8c96-96456ca62246.xml"}, "exchange direction": "INPUT", "other": {"anies": [{"name": "referenceToUnitGroupDataSet", "value": {"shortDescription": [{"value": "m^3", "lang": "en"}], "type": "unit group data set", "refObjectId": "cd950537-0a98-4044-9ba7-9f9a68d0a504", "uri": "../unitgroups/cd950537-0a98-4044-9ba7-9f9a68d0a504.xml"}}, {"value": "0.04182", "module": "A1-A3"}, {"value": "0.0001109", "module": "A4"}, {"value": "0.0048398", "module": "A5"}, {"value": "0", "module": "B1"}, {"value": "0.003344", "module": "B2"}, {"value": "0", "module": "C1"}, {"value": "6.23E-06", "module": "C2"}, {"value": "0.009008", "module": "C3", "scenario": "S2"}, {"value": "0.009129", "module": "C3", "scenario": "S3"}, {"value": "2.525E-05", "module": "C4"}, {"value": "-0.0005255", "module": "D", "scenario": "S0"}, {"value": "0", "module": "D", "scenario": "S1"}, {"value": "-0.003068", "module": "D", "scenario": "S2"}, {"value": "-0.002418", "module": "D", "scenario": "S3"}]}, "resolvedFlowVersion": "38.00.000", "flowProperties": [], "typeOfFlow": "Other flow", "classification": {"classHierarchy": "Quantities / Environmental quantities / EPD EN 15804 / LCI indicators", "name": "GaBiCategories"}}, {"dataSetInternalID": 11, "referenceToFlowDataSet": {"shortDescription": [{"value": "Hazardous waste disposed (HWD)", "lang": "en"}, {"value": "Gefährlicher Abfall zur Deponie (HWD)", "lang": "de"}], "type": "flow data set", "refObjectId": "430f9e0f-59b2-46a0-8e0d-55e0e84948fc", "uri": "../flows/430f9e0f-59b2-46a0-8e0d-55e0e84948fc.xml"}, "exchange direction": "OUTPUT", "other": {"anies": [{"name": "referenceToUnitGroupDataSet", "value": {"shortDescription": [{"value": "kg", "lang": "en"}], "type": "unit group data set", "refObjectId": "ad38d542-3fe9-439d-9b95-2f5f7752acaf", "uri": "../unitgroups/ad38d542-3fe9-439d-9b95-2f5f7752acaf.xml"}}, {"value": "0.000424", "module": "A1-A3"}, {"value": "8.29E-12", "module": "A4"}, {"value": "3.81600188E-05", "module": "A5"}, {"value": "0", "module": "B1"}, {"value": "4.19E-05", "module": "B2"}, {"value": "0", "module": "C1"}, {"value": "4.65E-13", "module": "C2"}, {"value": "1.86E-10", "module": "C3", "scenario": "S2"}, {"value": "2.04E-10", "module": "C3", "scenario": "S3"}, {"value": "3.33E-10", "module": "C4"}, {"value": "-2.72E-10", "module": "D", "scenario": "S0"}, {"value": "0", "module": "D", "scenario": "S1"}, {"value": "-1.61E-09", "module": "D", "scenario": "S2"}, {"value": "-1.37E-10", "module": "D", "scenario": "S3"}]}, "resolvedFlowVersion": "38.00.000", "flowProperties": [], "typeOfFlow": "Other flow", "classification": {"classHierarchy": "Quantities / Environmental quantities / EPD EN 15804 / LCI indicators", "name": "GaBiCategories"}}, {"dataSetInternalID": 12, "referenceToFlowDataSet": {"shortDescription": [{"value": "Non hazardous waste disposed (NHWD)", "lang": "en"}, {"value": "Entsorgter nicht gefährlicher Abfall (NHWD)", "lang": "de"}], "type": "flow data set", "refObjectId": "b29ef66b-e286-4afa-949f-62f1a7b4d7fa", "uri": "../flows/b29ef66b-e286-4afa-949f-62f1a7b4d7fa.xml"}, "exchange direction": "OUTPUT", "other": {"anies": [{"name": "referenceToUnitGroupDataSet", "value": {"shortDescription": [{"value": "kg", "lang": "en"}], "type": "unit group data set", "refObjectId": "ad38d542-3fe9-439d-9b95-2f5f7752acaf", "uri": "../unitgroups/ad38d542-3fe9-439d-9b95-2f5f7752acaf.xml"}}, {"value": "0.162", "module": "A1-A3"}, {"value": "0.000248", "module": "A4"}, {"value": "0.04668", "module": "A5"}, {"value": "0", "module": "B1"}, {"value": "0.0073", "module": "B2"}, {"value": "0", "module": "C1"}, {"value": "1.39E-05", "module": "C2"}, {"value": "0.351", "module": "C3", "scenario": "S2"}, {"value": "0.351", "module": "C3", "scenario": "S3"}, {"value": "2.14", "module": "C4"}, {"value": "-0.00101", "module": "D", "scenario": "S0"}, {"value": "0", "module": "D", "scenario": "S1"}, {"value": "-0.00594", "module": "D", "scenario": "S2"}, {"value": "-0.0705", "module": "D", "scenario": "S3"}]}, "resolvedFlowVersion": "38.00.000", "flowProperties": [], "typeOfFlow": "Other flow", "classification": {"classHierarchy": "Quantities / Environmental quantities / EPD EN 15804 / LCI indicators", "name": "GaBiCategories"}}, {"dataSetInternalID": 13, "referenceToFlowDataSet": {"shortDescription": [{"value": "Radioactive waste disposed (RWD)", "lang": "en"}, {"value": "Entsorgter radioaktiver Abfall (RWD)", "lang": "de"}], "type": "flow data set", "refObjectId": "3449546e-52ad-4b39-b809-9fb77cea8ff6", "uri": "../flows/3449546e-52ad-4b39-b809-9fb77cea8ff6.xml"}, "exchange direction": "OUTPUT", "other": {"anies": [{"name": "referenceToUnitGroupDataSet", "value": {"shortDescription": [{"value": "kg", "lang": "en"}], "type": "unit group data set", "refObjectId": "ad38d542-3fe9-439d-9b95-2f5f7752acaf", "uri": "../unitgroups/ad38d542-3fe9-439d-9b95-2f5f7752acaf.xml"}}, {"value": "0.00414", "module": "A1-A3"}, {"value": "2.13E-06", "module": "A4"}, {"value": "0.00037842", "module": "A5"}, {"value": "0", "module": "B1"}, {"value": "0.000376", "module": "B2"}, {"value": "0", "module": "C1"}, {"value": "1.2E-07", "module": "C2"}, {"value": "5.32E-05", "module": "C3", "scenario": "S2"}, {"value": "8.53E-05", "module": "C3", "scenario": "S3"}, {"value": "2.65E-05", "module": "C4"}, {"value": "-0.000158", "module": "D", "scenario": "S0"}, {"value": "0", "module": "D", "scenario": "S1"}, {"value": "-0.000921", "module": "D", "scenario": "S2"}, {"value": "-6E-05", "module": "D", "scenario": "S3"}]}, "resolvedFlowVersion": "38.00.000", "flowProperties": [], "typeOfFlow": "Other flow", "classification": {"classHierarchy": "Quantities / Environmental quantities / EPD EN 15804 / LCI indicators", "name": "GaBiCategories"}}, {"dataSetInternalID": 14, "referenceToFlowDataSet": {"shortDescription": [{"value": "Components for re-use (CRU)", "lang": "en"}, {"value": "Komponenten für die Wiederverwendung (CRU)", "lang": "de"}], "type": "flow data set", "refObjectId": "a2b32f97-3fc7-4af2-b209-525bc6426f33", "uri": "../flows/a2b32f97-3fc7-4af2-b209-525bc6426f33.xml"}, "exchange direction": "OUTPUT", "other": {"anies": [{"name": "referenceToUnitGroupDataSet", "value": {"shortDescription": [{"value": "kg", "lang": "en"}], "type": "unit group data set", "refObjectId": "ad38d542-3fe9-439d-9b95-2f5f7752acaf", "uri": "../unitgroups/ad38d542-3fe9-439d-9b95-2f5f7752acaf.xml"}}, {"value": "0", "module": "A1-A3"}, {"value": "0", "module": "A4"}, {"value": "0", "module": "A5"}, {"value": "0", "module": "B1"}, {"value": "0", "module": "B2"}, {"value": "0", "module": "C1"}, {"value": "0", "module": "C2"}, {"value": "0", "module": "C3", "scenario": "S2"}, {"value": "0", "module": "C3", "scenario": "S3"}, {"value": "0", "module": "C4"}, {"value": "0", "module": "D", "scenario": "S0"}, {"value": "0", "module": "D", "scenario": "S1"}, {"value": "0", "module": "D", "scenario": "S2"}, {"value": "0", "module": "D", "scenario": "S3"}]}, "resolvedFlowVersion": "38.00.000", "flowProperties": [], "typeOfFlow": "Other flow", "classification": {"classHierarchy": "Quantities / Environmental quantities / EPD EN 15804 / LCI indicators", "name": "GaBiCategories"}}, {"dataSetInternalID": 15, "referenceToFlowDataSet": {"shortDescription": [{"value": "Materials for recycling (MFR)", "lang": "en"}, {"value": "Stoffe zum Recycling (MFR)", "lang": "de"}], "type": "flow data set", "refObjectId": "d7fe48a5-4103-49c8-9aae-b0b5dfdbd6ae", "uri": "../flows/d7fe48a5-4103-49c8-9aae-b0b5dfdbd6ae.xml"}, "exchange direction": "OUTPUT", "other": {"anies": [{"name": "referenceToUnitGroupDataSet", "value": {"shortDescription": [{"value": "kg", "lang": "en"}], "type": "unit group data set", "refObjectId": "ad38d542-3fe9-439d-9b95-2f5f7752acaf", "uri": "../unitgroups/ad38d542-3fe9-439d-9b95-2f5f7752acaf.xml"}}, {"value": "0", "module": "A1-A3"}, {"value": "0", "module": "A4"}, {"value": "0", "module": "A5"}, {"value": "0", "module": "B1"}, {"value": "0", "module": "B2"}, {"value": "0", "module": "C1"}, {"value": "0", "module": "C2"}, {"value": "0", "module": "C3", "scenario": "S2"}, {"value": "0.34", "module": "C3", "scenario": "S3"}, {"value": "0", "module": "C4"}, {"value": "0", "module": "D", "scenario": "S0"}, {"value": "0", "module": "D", "scenario": "S1"}, {"value": "0", "module": "D", "scenario": "S2"}, {"value": "0", "module": "D", "scenario": "S3"}]}, "resolvedFlowVersion": "38.00.000", "flowProperties": [], "typeOfFlow": "Other flow", "classification": {"classHierarchy": "Quantities / Environmental quantities / EPD EN 15804 / LCI indicators", "name": "GaBiCategories"}}, {"dataSetInternalID": 16, "referenceToFlowDataSet": {"shortDescription": [{"value": "Materials for energy recovery (MER)", "lang": "en"}, {"value": "Stoffe für die Energierückgewinnung (MER)", "lang": "de"}], "type": "flow data set", "refObjectId": "59a9181c-3aaf-46ee-8b13-2b3723b6e447", "uri": "../flows/59a9181c-3aaf-46ee-8b13-2b3723b6e447.xml"}, "exchange direction": "OUTPUT", "other": {"anies": [{"name": "referenceToUnitGroupDataSet", "value": {"shortDescription": [{"value": "kg", "lang": "en"}], "type": "unit group data set", "refObjectId": "ad38d542-3fe9-439d-9b95-2f5f7752acaf", "uri": "../unitgroups/ad38d542-3fe9-439d-9b95-2f5f7752acaf.xml"}}, {"value": "0", "module": "A1-A3"}, {"value": "0", "module": "A4"}, {"value": "0", "module": "A5"}, {"value": "0", "module": "B1"}, {"value": "0", "module": "B2"}, {"value": "0", "module": "C1"}, {"value": "0", "module": "C2"}, {"value": "0", "module": "C3", "scenario": "S2"}, {"value": "0", "module": "C3", "scenario": "S3"}, {"value": "0", "module": "C4"}, {"value": "0", "module": "D", "scenario": "S0"}, {"value": "0", "module": "D", "scenario": "S1"}, {"value": "0", "module": "D", "scenario": "S2"}, {"value": "0", "module": "D", "scenario": "S3"}]}, "resolvedFlowVersion": "38.00.000", "flowProperties": [], "typeOfFlow": "Other flow", "classification": {"classHierarchy": "Quantities / Environmental quantities / EPD EN 15804 / LCI indicators", "name": "GaBiCategories"}}, {"dataSetInternalID": 17, "referenceToFlowDataSet": {"shortDescription": [{"value": "Exported electrical energy (EEE)", "lang": "en"}, {"value": "Exportierte elektrische Energie (EEE)", "lang": "de"}], "type": "flow data set", "refObjectId": "4da0c987-2b76-40d6-9e9e-82a017aaaf29", "uri": "../flows/4da0c987-2b76-40d6-9e9e-82a017aaaf29.xml"}, "exchange direction": "OUTPUT", "other": {"anies": [{"name": "referenceToUnitGroupDataSet", "value": {"shortDescription": [{"value": "MJ", "lang": "en"}], "type": "unit group data set", "refObjectId": "93a60a57-a3c8-11da-a746-0800200c9a66", "uri": "../unitgroups/93a60a57-a3c8-11da-a746-0800200c9a66.xml"}}, {"value": "0", "module": "A1-A3"}, {"value": "0", "module": "A4"}, {"value": "0.677", "module": "A5"}, {"value": "0", "module": "B1"}, {"value": "0", "module": "B2"}, {"value": "0", "module": "C1"}, {"value": "0", "module": "C2"}, {"value": "4.73", "module": "C3", "scenario": "S2"}, {"value": "0", "module": "C3", "scenario": "S3"}, {"value": "0", "module": "C4"}, {"value": "0", "module": "D", "scenario": "S0"}, {"value": "0", "module": "D", "scenario": "S1"}, {"value": "0", "module": "D", "scenario": "S2"}, {"value": "0", "module": "D", "scenario": "S3"}]}, "resolvedFlowVersion": "38.00.000", "flowProperties": [], "typeOfFlow": "Other flow", "classification": {"classHierarchy": "Quantities / Environmental quantities / EPD EN 15804 / LCI indicators", "name": "GaBiCategories"}}, {"dataSetInternalID": 18, "referenceToFlowDataSet": {"shortDescription": [{"value": "Exported thermal energy (EET)", "lang": "en"}, {"value": "Exportierte thermische Energie (EET)", "lang": "de"}], "type": "flow data set", "refObjectId": "98daf38a-7a79-46d3-9a37-2b7bd0955810", "uri": "../flows/98daf38a-7a79-46d3-9a37-2b7bd0955810.xml"}, "exchange direction": "OUTPUT", "other": {"anies": [{"name": "referenceToUnitGroupDataSet", "value": {"shortDescription": [{"value": "MJ", "lang": "en"}], "type": "unit group data set", "refObjectId": "93a60a57-a3c8-11da-a746-0800200c9a66", "uri": "../unitgroups/93a60a57-a3c8-11da-a746-0800200c9a66.xml"}}, {"value": "0", "module": "A1-A3"}, {"value": "0", "module": "A4"}, {"value": "1.22", "module": "A5"}, {"value": "0", "module": "B1"}, {"value": "0", "module": "B2"}, {"value": "0", "module": "C1"}, {"value": "0", "module": "C2"}, {"value": "8.64", "module": "C3", "scenario": "S2"}, {"value": "40.6", "module": "C3", "scenario": "S3"}, {"value": "0", "module": "C4"}, {"value": "0", "module": "D", "scenario": "S0"}, {"value": "0", "module": "D", "scenario": "S1"}, {"value": "0", "module": "D", "scenario": "S2"}, {"value": "0", "module": "D", "scenario": "S3"}]}, "resolvedFlowVersion": "38.00.000", "flowProperties": [], "typeOfFlow": "Other flow", "classification": {"classHierarchy": "Quantities / Environmental quantities / EPD EN 15804 / LCI indicators", "name": "GaBiCategories"}}]}, "LCIAResults": {"LCIAResult": [{"referenceToLCIAMethodDataSet": {"shortDescription": [{"value": "Global Warming Potential total (GWP-total)", "lang": "en"}, {"value": "Globales Erwärmungspotenzial total (GWP-total)", "lang": "de"}], "type": "LCIA method data set", "refObjectId": "6a37f984-a4b3-458a-a20a-64418c145fa2", "uri": "../lciamethods/6a37f984-a4b3-458a-a20a-64418c145fa2.xml"}, "other": {"anies": [{"name": "referenceToUnitGroupDataSet", "value": {"shortDescription": [{"value": "kg CO_(2) eq", "lang": "en"}], "type": "unit group data set", "refObjectId": "1ebf3012-d0db-4de2-aefd-ef30cedb0be1", "uri": "../unitgroups/1ebf3012-d0db-4de2-aefd-ef30cedb0be1.xml"}}, {"value": "8.128", "module": "A1-A3"}, {"value": "0.1296", "module": "A4"}, {"value": "1.16632", "module": "A5"}, {"value": "0", "module": "B1"}, {"value": "0.5488", "module": "B2"}, {"value": "0", "module": "C1"}, {"value": "0.007277", "module": "C2"}, {"value": "3.386", "module": "C3", "scenario": "S2"}, {"value": "3.416", "module": "C3", "scenario": "S3"}, {"value": "0.1504", "module": "C4"}, {"value": "-0.1188", "module": "D", "scenario": "S0"}, {"value": "0", "module": "D", "scenario": "S1"}, {"value": "-0.6998", "module": "D", "scenario": "S2"}, {"value": "-0.2072", "module": "D", "scenario": "S3"}]}}, {"referenceToLCIAMethodDataSet": {"shortDescription": [{"value": "Global Warming Potential fossil fuels (GWP-fossil)", "lang": "en"}, {"value": "Globales Erwärmungspotenzial fossil (GWP-fossil)", "lang": "de"}], "type": "LCIA method data set", "refObjectId": "5f635281-343e-44fb-83df-1971b155e6b6", "uri": "../lciamethods/5f635281-343e-44fb-83df-1971b155e6b6.xml"}, "other": {"anies": [{"name": "referenceToUnitGroupDataSet", "value": {"shortDescription": [{"value": "kg CO_(2) eq", "lang": "en"}], "type": "unit group data set", "refObjectId": "1ebf3012-d0db-4de2-aefd-ef30cedb0be1", "uri": "../unitgroups/1ebf3012-d0db-4de2-aefd-ef30cedb0be1.xml"}}, {"value": "8.047", "module": "A1-A3"}, {"value": "0.1272", "module": "A4"}, {"value": "1.15873", "module": "A5"}, {"value": "0", "module": "B1"}, {"value": "0.3484", "module": "B2"}, {"value": "0", "module": "C1"}, {"value": "0.007144", "module": "C2"}, {"value": "3.386", "module": "C3", "scenario": "S2"}, {"value": "3.415", "module": "C3", "scenario": "S3"}, {"value": "0.1503", "module": "C4"}, {"value": "-0.1182", "module": "D", "scenario": "S0"}, {"value": "0", "module": "D", "scenario": "S1"}, {"value": "-0.6962", "module": "D", "scenario": "S2"}, {"value": "-0.2068", "module": "D", "scenario": "S3"}]}}, {"referenceToLCIAMethodDataSet": {"shortDescription": [{"value": "Global Warming Potential biogenic (GWP-biogenic)", "lang": "en"}, {"value": "Globales Erwärmungspotenzial biogen (GWP-biogenic)", "lang": "de"}], "type": "LCIA method data set", "refObjectId": "2356e1ab-0185-4db5-86e5-16de51c7485c", "uri": "../lciamethods/2356e1ab-0185-4db5-86e5-16de51c7485c.xml"}, "other": {"anies": [{"name": "referenceToUnitGroupDataSet", "value": {"shortDescription": [{"value": "kg CO_(2) eq", "lang": "en"}], "type": "unit group data set", "refObjectId": "1ebf3012-d0db-4de2-aefd-ef30cedb0be1", "uri": "../unitgroups/1ebf3012-d0db-4de2-aefd-ef30cedb0be1.xml"}}, {"value": "0.07791", "module": "A1-A3"}, {"value": "0.001647", "module": "A4"}, {"value": "0.0071995", "module": "A5"}, {"value": "0", "module": "B1"}, {"value": "0.004159", "module": "B2"}, {"value": "0", "module": "C1"}, {"value": "9.246E-05", "module": "C2"}, {"value": "0.0003145", "module": "C3", "scenario": "S2"}, {"value": "0.0006445", "module": "C3", "scenario": "S3"}, {"value": "-2.47E-08", "module": "C4"}, {"value": "-0.000603", "module": "D", "scenario": "S0"}, {"value": "0", "module": "D", "scenario": "S1"}, {"value": "-0.003532", "module": "D", "scenario": "S2"}, {"value": "-0.0002493", "module": "D", "scenario": "S3"}]}}, {"referenceToLCIAMethodDataSet": {"shortDescription": [{"value": "Global Warming Potential luluc (GWP-luluc)", "lang": "en"}, {"value": "Globales Erwärmungspotenzial luluc (GWP-luluc)", "lang": "de"}], "type": "LCIA method data set", "refObjectId": "4331bbdb-978a-490d-8707-eeb047f01a55", "uri": "../lciamethods/4331bbdb-978a-490d-8707-eeb047f01a55.xml"}, "other": {"anies": [{"name": "referenceToUnitGroupDataSet", "value": {"shortDescription": [{"value": "kg CO_(2) eq", "lang": "en"}], "type": "unit group data set", "refObjectId": "1ebf3012-d0db-4de2-aefd-ef30cedb0be1", "uri": "../unitgroups/1ebf3012-d0db-4de2-aefd-ef30cedb0be1.xml"}}, {"value": "0.003448", "module": "A1-A3"}, {"value": "0.0007204", "module": "A4"}, {"value": "0.00038475", "module": "A5"}, {"value": "0", "module": "B1"}, {"value": "0.1962", "module": "B2"}, {"value": "0", "module": "C1"}, {"value": "4.046E-05", "module": "C2"}, {"value": "6.951E-05", "module": "C3", "scenario": "S2"}, {"value": "0.000173", "module": "C3", "scenario": "S3"}, {"value": "7.398E-05", "module": "C4"}, {"value": "-1.295E-05", "module": "D", "scenario": "S0"}, {"value": "0", "module": "D", "scenario": "S1"}, {"value": "-7.575E-05", "module": "D", "scenario": "S2"}, {"value": "-9.994E-05", "module": "D", "scenario": "S3"}]}}, {"referenceToLCIAMethodDataSet": {"shortDescription": [{"value": "Depletion potential of the stratospheric ozone layer (ODP)", "lang": "en"}, {"value": "Abbau Potential der stratosphärischen Ozonschicht (ODP)", "lang": "de"}], "type": "LCIA method data set", "refObjectId": "b5c629d6-def3-11e6-bf01-fe55135034f3", "uri": "../lciamethods/b5c629d6-def3-11e6-bf01-fe55135034f3.xml"}, "other": {"anies": [{"name": "referenceToUnitGroupDataSet", "value": {"shortDescription": [{"value": "kg CFC11 eq", "lang": "en"}], "type": "unit group data set", "refObjectId": "d9e957c9-7309-4474-bf3a-7777df6c4e5b", "uri": "../unitgroups/d9e957c9-7309-4474-bf3a-7777df6c4e5b.xml"}}, {"value": "4.4E-09", "module": "A1-A3"}, {"value": "7.742E-15", "module": "A4"}, {"value": "3.9603034E-10", "module": "A5"}, {"value": "0", "module": "B1"}, {"value": "3.415E-08", "module": "B2"}, {"value": "0", "module": "C1"}, {"value": "4.348E-16", "module": "C2"}, {"value": "2.73E-13", "module": "C3", "scenario": "S2"}, {"value": "4.348E-13", "module": "C3", "scenario": "S3"}, {"value": "2.041E-13", "module": "C4"}, {"value": "-7.959E-13", "module": "D", "scenario": "S0"}, {"value": "0", "module": "D", "scenario": "S1"}, {"value": "-4.647E-12", "module": "D", "scenario": "S2"}, {"value": "-3.119E-13", "module": "D", "scenario": "S3"}]}}, {"referenceToLCIAMethodDataSet": {"shortDescription": [{"value": "Acidification potential of land and water (AP)", "lang": "en"}, {"value": "Versauerungspotenzial von Boden und Wasser (AP)", "lang": "de"}], "type": "LCIA method data set", "refObjectId": "b5c611c6-def3-11e6-bf01-fe55135034f3", "uri": "../lciamethods/b5c611c6-def3-11e6-bf01-fe55135034f3.xml"}, "other": {"anies": [{"name": "referenceToUnitGroupDataSet", "value": {"shortDescription": [{"value": "mol H^(+) eq", "lang": "en"}], "type": "unit group data set", "refObjectId": "42e089ac-92bf-4bf2-8ca1-5fc40d18f2ed", "uri": "../unitgroups/42e089ac-92bf-4bf2-8ca1-5fc40d18f2ed.xml"}}, {"value": "0.01365", "module": "A1-A3"}, {"value": "0.0007693", "module": "A4"}, {"value": "0.0015104", "module": "A5"}, {"value": "0", "module": "B1"}, {"value": "0.000832", "module": "B2"}, {"value": "0", "module": "C1"}, {"value": "4.32E-05", "module": "C2"}, {"value": "0.002194", "module": "C3", "scenario": "S2"}, {"value": "0.002326", "module": "C3", "scenario": "S3"}, {"value": "0.0004504", "module": "C4"}, {"value": "-0.0001551", "module": "D", "scenario": "S0"}, {"value": "0", "module": "D", "scenario": "S1"}, {"value": "-0.0009091", "module": "D", "scenario": "S2"}, {"value": "-0.0007403", "module": "D", "scenario": "S3"}]}}, {"referenceToLCIAMethodDataSet": {"shortDescription": [{"value": "Eutrophication potential aquatic freshwater (EP-freshwater)", "lang": "en"}, {"value": "Eutrophierungspotenzial Süßwasser (EP-freshwater)", "lang": "de"}], "type": "LCIA method data set", "refObjectId": "b53ec18f-7377-4ad3-86eb-cc3f4f276b2b", "uri": "../lciamethods/b53ec18f-7377-4ad3-86eb-cc3f4f276b2b.xml"}, "other": {"anies": [{"name": "referenceToUnitGroupDataSet", "value": {"shortDescription": [{"value": "kg P eq", "lang": "en"}], "type": "unit group data set", "refObjectId": "0429039d-a61d-4590-ba67-aa4a20a810a1", "uri": "../unitgroups/0429039d-a61d-4590-ba67-aa4a20a810a1.xml"}}, {"value": "4.129E-05", "module": "A1-A3"}, {"value": "3.857E-07", "module": "A4"}, {"value": "3.77882E-06", "module": "A5"}, {"value": "0", "module": "B1"}, {"value": "5.189E-06", "module": "B2"}, {"value": "0", "module": "C1"}, {"value": "2.166E-08", "module": "C2"}, {"value": "2.789E-07", "module": "C3", "scenario": "S2"}, {"value": "3.651E-07", "module": "C3", "scenario": "S3"}, {"value": "2.837E-05", "module": "C4"}, {"value": "-1.62E-07", "module": "D", "scenario": "S0"}, {"value": "0", "module": "D", "scenario": "S1"}, {"value": "-9.461E-07", "module": "D", "scenario": "S2"}, {"value": "-2.327E-07", "module": "D", "scenario": "S3"}]}}, {"referenceToLCIAMethodDataSet": {"shortDescription": [{"value": "Eutrophication potential aquatic marine (EP-marine)", "lang": "en"}, {"value": "Eutrophierungspotenzial Salzwasser (EP-marine)", "lang": "de"}], "type": "LCIA method data set", "refObjectId": "b5c619fa-def3-11e6-bf01-fe55135034f3", "uri": "../lciamethods/b5c619fa-def3-11e6-bf01-fe55135034f3.xml"}, "other": {"anies": [{"name": "referenceToUnitGroupDataSet", "value": {"shortDescription": [{"value": "kg N eq", "lang": "en"}], "type": "unit group data set", "refObjectId": "d05bb823-ecdf-4686-8c40-bf1d9257859f", "uri": "../unitgroups/d05bb823-ecdf-4686-8c40-bf1d9257859f.xml"}}, {"value": "0.004183", "module": "A1-A3"}, {"value": "0.0003777", "module": "A4"}, {"value": "0.00050877", "module": "A5"}, {"value": "0", "module": "B1"}, {"value": "0.000197", "module": "B2"}, {"value": "0", "module": "C1"}, {"value": "2.121E-05", "module": "C2"}, {"value": "0.001046", "module": "C3", "scenario": "S2"}, {"value": "0.001105", "module": "C3", "scenario": "S3"}, {"value": "9.963E-05", "module": "C4"}, {"value": "-4.212E-05", "module": "D", "scenario": "S0"}, {"value": "0", "module": "D", "scenario": "S1"}, {"value": "-0.0002474", "module": "D", "scenario": "S2"}, {"value": "-0.0002304", "module": "D", "scenario": "S3"}]}}, {"referenceToLCIAMethodDataSet": {"shortDescription": [{"value": "Eutrophication potential terrestrial (EP-terrestrial)", "lang": "en"}, {"value": "Eutrophierungspotenzial Land (EP-terrestrial)", "lang": "de"}], "type": "LCIA method data set", "refObjectId": "b5c614d2-def3-11e6-bf01-fe55135034f3", "uri": "../lciamethods/b5c614d2-def3-11e6-bf01-fe55135034f3.xml"}, "other": {"anies": [{"name": "referenceToUnitGroupDataSet", "value": {"shortDescription": [{"value": "mol N eq", "lang": "en"}], "type": "unit group data set", "refObjectId": "71b4d617-0ec9-4d3f-b65e-e438940c2401", "uri": "../unitgroups/71b4d617-0ec9-4d3f-b65e-e438940c2401.xml"}}, {"value": "0.04071", "module": "A1-A3"}, {"value": "0.004181", "module": "A4"}, {"value": "0.0051819", "module": "A5"}, {"value": "0", "module": "B1"}, {"value": "0.002831", "module": "B2"}, {"value": "0", "module": "C1"}, {"value": "0.0002348", "module": "C2"}, {"value": "0.01187", "module": "C3", "scenario": "S2"}, {"value": "0.01252", "module": "C3", "scenario": "S3"}, {"value": "0.001093", "module": "C4"}, {"value": "-0.0004512", "module": "D", "scenario": "S0"}, {"value": "0", "module": "D", "scenario": "S1"}, {"value": "-0.002651", "module": "D", "scenario": "S2"}, {"value": "-0.002525", "module": "D", "scenario": "S3"}]}}, {"referenceToLCIAMethodDataSet": {"shortDescription": [{"value": "Formation potential of tropospheric ozone photochemical oxidants (POCP)", "lang": "en"}, {"value": "Bildungspotential für troposphärisches Ozon (POCP)", "lang": "de"}], "type": "LCIA method data set", "refObjectId": "b5c610fe-def3-11e6-bf01-fe55135034f3", "uri": "../lciamethods/b5c610fe-def3-11e6-bf01-fe55135034f3.xml"}, "other": {"anies": [{"name": "referenceToUnitGroupDataSet", "value": {"shortDescription": [{"value": "kg NMVOC eq", "lang": "en"}], "type": "unit group data set", "refObjectId": "d27c25f8-fbc1-44c6-b47b-4adbae4199c6", "uri": "../unitgroups/d27c25f8-fbc1-44c6-b47b-4adbae4199c6.xml"}}, {"value": "0.01324", "module": "A1-A3"}, {"value": "0.000714", "module": "A4"}, {"value": "0.0015085", "module": "A5"}, {"value": "0.000418", "module": "B1"}, {"value": "0.0009833", "module": "B2"}, {"value": "0", "module": "C1"}, {"value": "4.01E-05", "module": "C2"}, {"value": "0.002691", "module": "C3", "scenario": "S2"}, {"value": "0.002806", "module": "C3", "scenario": "S3"}, {"value": "0.0003205", "module": "C4"}, {"value": "-0.0001179", "module": "D", "scenario": "S0"}, {"value": "0", "module": "D", "scenario": "S1"}, {"value": "-0.0006928", "module": "D", "scenario": "S2"}, {"value": "-0.0006931", "module": "D", "scenario": "S3"}]}}, {"referenceToLCIAMethodDataSet": {"shortDescription": [{"value": "Abiotic depletion potential for non fossil resources (ADPE)", "lang": "en"}, {"value": "Potenzial für den abiotischen Abbau nicht fossiler Ressourcen (ADPE)", "lang": "de"}], "type": "LCIA method data set", "refObjectId": "b2ad6494-c78d-11e6-9d9d-cec0c932ce01", "uri": "../lciamethods/b2ad6494-c78d-11e6-9d9d-cec0c932ce01.xml"}, "other": {"anies": [{"name": "referenceToUnitGroupDataSet", "value": {"shortDescription": [{"value": "kg Sb eq", "lang": "en"}], "type": "unit group data set", "refObjectId": "54ccd2d9-a32a-4fc2-923d-f2c8c93e89d4", "uri": "../unitgroups/54ccd2d9-a32a-4fc2-923d-f2c8c93e89d4.xml"}}, {"value": "1.36E-06", "module": "A1-A3"}, {"value": "1.08E-08", "module": "A4"}, {"value": "1.2455E-07", "module": "A5"}, {"value": "0", "module": "B1"}, {"value": "2.301E-07", "module": "B2"}, {"value": "0", "module": "C1"}, {"value": "6.066E-10", "module": "C2"}, {"value": "1.119E-08", "module": "C3", "scenario": "S2"}, {"value": "1.57E-08", "module": "C3", "scenario": "S3"}, {"value": "1.054E-08", "module": "C4"}, {"value": "-1.778E-08", "module": "D", "scenario": "S0"}, {"value": "0", "module": "D", "scenario": "S1"}, {"value": "-1.041E-07", "module": "D", "scenario": "S2"}, {"value": "-1.989E-08", "module": "D", "scenario": "S3"}]}}, {"referenceToLCIAMethodDataSet": {"shortDescription": [{"value": "Abiotic depletion potential for fossil resources (ADPF)", "lang": "en"}, {"value": "Potenzial für den abiotischen Abbau fossiler Brennstoffe (ADPF)", "lang": "de"}], "type": "LCIA method data set", "refObjectId": "b2ad6110-c78d-11e6-9d9d-cec0c932ce01", "uri": "../lciamethods/b2ad6110-c78d-11e6-9d9d-cec0c932ce01.xml"}, "other": {"anies": [{"name": "referenceToUnitGroupDataSet", "value": {"shortDescription": [{"value": "MJ", "lang": "en"}], "type": "unit group data set", "refObjectId": "93a60a57-a3c8-11da-a746-0800200c9a66", "uri": "../unitgroups/93a60a57-a3c8-11da-a746-0800200c9a66.xml"}}, {"value": "159.1", "module": "A1-A3"}, {"value": "1.727", "module": "A4"}, {"value": "14.6158", "module": "A5"}, {"value": "0", "module": "B1"}, {"value": "5.897", "module": "B2"}, {"value": "0", "module": "C1"}, {"value": "0.09697", "module": "C2"}, {"value": "1.332", "module": "C3", "scenario": "S2"}, {"value": "1.774", "module": "C3", "scenario": "S3"}, {"value": "2.156", "module": "C4"}, {"value": "-2.01", "module": "D", "scenario": "S0"}, {"value": "0", "module": "D", "scenario": "S1"}, {"value": "-11.83", "module": "D", "scenario": "S2"}, {"value": "-26.43", "module": "D", "scenario": "S3"}]}}, {"referenceToLCIAMethodDataSet": {"shortDescription": [{"value": "Water use (WDP)", "lang": "en"}, {"value": "Wassernutzung (WDP)", "lang": "de"}], "type": "LCIA method data set", "refObjectId": "b2ad66ce-c78d-11e6-9d9d-cec0c932ce01", "uri": "../lciamethods/b2ad66ce-c78d-11e6-9d9d-cec0c932ce01.xml"}, "other": {"anies": [{"name": "referenceToUnitGroupDataSet", "value": {"shortDescription": [{"value": "m^(3) world eq deprived", "lang": "en"}], "type": "unit group data set", "refObjectId": "6ae2df01-888e-46c8-b17d-49fa3869b476", "uri": "../unitgroups/6ae2df01-888e-46c8-b17d-49fa3869b476.xml"}}, {"value": "1.043", "module": "A1-A3"}, {"value": "0.001156", "module": "A4"}, {"value": "0.1392", "module": "A5"}, {"value": "0", "module": "B1"}, {"value": "0.09986", "module": "B2"}, {"value": "0", "module": "C1"}, {"value": "6.49E-05", "module": "C2"}, {"value": "0.3818", "module": "C3", "scenario": "S2"}, {"value": "0.3844", "module": "C3", "scenario": "S3"}, {"value": "-0.001612", "module": "C4"}, {"value": "-0.0124", "module": "D", "scenario": "S0"}, {"value": "0", "module": "D", "scenario": "S1"}, {"value": "-0.07243", "module": "D", "scenario": "S2"}, {"value": "-0.03078", "module": "D", "scenario": "S3"}]}}, {"referenceToLCIAMethodDataSet": {"shortDescription": [{"value": "Incidence of disease due to PM emissions (PM)", "lang": "en"}, {"value": "Auftreten von Krankheiten aufgrund von Feinstaubemissionen (PM)", "lang": "de"}], "type": "LCIA method data set", "refObjectId": "b5c602c6-def3-11e6-bf01-fe55135034f3", "uri": "../lciamethods/b5c602c6-def3-11e6-bf01-fe55135034f3.xml"}, "other": {"anies": [{"name": "referenceToUnitGroupDataSet", "value": {"shortDescription": [{"value": "Disease incidence", "lang": "en"}], "type": "unit group data set", "refObjectId": "3883559b-648f-4afc-8ba2-0bd24f3affa3", "uri": "../unitgroups/3883559b-648f-4afc-8ba2-0bd24f3affa3.xml"}}, {"value": "9.59E-08", "module": "A1-A3"}, {"value": "4.45E-09", "module": "A4"}, {"value": "9.951E-09", "module": "A5"}, {"value": "0", "module": "B1"}, {"value": "6.84E-08", "module": "B2"}, {"value": "0", "module": "C1"}, {"value": "2.5E-10", "module": "C2"}, {"value": "9.2E-09", "module": "C3", "scenario": "S2"}, {"value": "1E-08", "module": "C3", "scenario": "S3"}, {"value": "4.33E-09", "module": "C4"}, {"value": "-1.28E-09", "module": "D", "scenario": "S0"}, {"value": "0", "module": "D", "scenario": "S1"}, {"value": "0", "module": "D", "scenario": "S2"}, {"value": "-1.37E-08", "module": "D", "scenario": "S3"}]}}, {"referenceToLCIAMethodDataSet": {"shortDescription": [{"value": "Human exposure efficiency relative to U235 (IR)", "lang": "en"}, {"value": "Wirkung durch Exposition des Menschen mit U235 (IR)", "lang": "de"}], "type": "LCIA method data set", "refObjectId": "b5c632be-def3-11e6-bf01-fe55135034f3", "uri": "../lciamethods/b5c632be-def3-11e6-bf01-fe55135034f3.xml"}, "other": {"anies": [{"name": "referenceToUnitGroupDataSet", "value": {"shortDescription": [{"value": "kBq U235 eq", "lang": "en"}], "type": "unit group data set", "refObjectId": "456b05bf-1415-44a9-9993-02452f554c09", "uri": "../unitgroups/456b05bf-1415-44a9-9993-02452f554c09.xml"}}, {"value": "0.684", "module": "A1-A3"}, {"value": "0.000312", "module": "A4"}, {"value": "0.06247", "module": "A5"}, {"value": "0", "module": "B1"}, {"value": "0.0678", "module": "B2"}, {"value": "0", "module": "C1"}, {"value": "1.75E-05", "module": "C2"}, {"value": "0.00827", "module": "C3", "scenario": "S2"}, {"value": "0.0137", "module": "C3", "scenario": "S3"}, {"value": "0.00391", "module": "C4"}, {"value": "-0.0267", "module": "D", "scenario": "S0"}, {"value": "0", "module": "D", "scenario": "S1"}, {"value": "0", "module": "D", "scenario": "S2"}, {"value": "-0.00671", "module": "D", "scenario": "S3"}]}}, {"referenceToLCIAMethodDataSet": {"shortDescription": [{"value": "Comparative toxic unit for ecosystems (ETP-fw)", "lang": "en"}, {"value": "Toxizitätsvergleichseinheit für Ökosysteme (ETP-fw)", "lang": "de"}], "type": "LCIA method data set", "refObjectId": "ee1082d1-b0f7-43ca-a1f0-21e2a4a74511", "uri": "../lciamethods/ee1082d1-b0f7-43ca-a1f0-21e2a4a74511.xml"}, "other": {"anies": [{"name": "referenceToUnitGroupDataSet", "value": {"shortDescription": [{"value": "CTUe", "lang": "en"}], "type": "unit group data set", "refObjectId": "aa959ded-f1eb-4efb-9c5c-2d60be36b3e6", "uri": "../unitgroups/aa959ded-f1eb-4efb-9c5c-2d60be36b3e6.xml"}}, {"value": "72", "module": "A1-A3"}, {"value": "1.2", "module": "A4"}, {"value": "6.656", "module": "A5"}, {"value": "0.0036", "module": "B1"}, {"value": "2.69", "module": "B2"}, {"value": "0", "module": "C1"}, {"value": "0.0673", "module": "C2"}, {"value": "0.627", "module": "C3", "scenario": "S2"}, {"value": "0.883", "module": "C3", "scenario": "S3"}, {"value": "2.11", "module": "C4"}, {"value": "-0.44", "module": "D", "scenario": "S0"}, {"value": "0", "module": "D", "scenario": "S1"}, {"value": "0", "module": "D", "scenario": "S2"}, {"value": "-4.67", "module": "D", "scenario": "S3"}]}}, {"referenceToLCIAMethodDataSet": {"shortDescription": [{"value": "Comparative toxic unit for humans (carcinogenic) (HTP-c)", "lang": "en"}, {"value": "Toxizitätsvergleichseinheit für Menschen (krebserregend) (HTP-c)", "lang": "de"}], "type": "LCIA method data set", "refObjectId": "2299222a-bbd8-474f-9d4f-4dd1f18aea7c", "uri": "../lciamethods/2299222a-bbd8-474f-9d4f-4dd1f18aea7c.xml"}, "other": {"anies": [{"name": "referenceToUnitGroupDataSet", "value": {"shortDescription": [{"value": "CTUh", "lang": "en"}], "type": "unit group data set", "refObjectId": "d4c9523e-2d7e-49fd-8469-998f547d3a70", "uri": "../unitgroups/d4c9523e-2d7e-49fd-8469-998f547d3a70.xml"}}, {"value": "2.64E-09", "module": "A1-A3"}, {"value": "2.42E-11", "module": "A4"}, {"value": "2.4382E-10", "module": "A5"}, {"value": "0", "module": "B1"}, {"value": "6.21E-10", "module": "B2"}, {"value": "0", "module": "C1"}, {"value": "1.36E-12", "module": "C2"}, {"value": "3.53E-11", "module": "C3", "scenario": "S2"}, {"value": "4.12E-11", "module": "C3", "scenario": "S3"}, {"value": "9.48E-11", "module": "C4"}, {"value": "-2.03E-11", "module": "D", "scenario": "S0"}, {"value": "0", "module": "D", "scenario": "S1"}, {"value": "0", "module": "D", "scenario": "S2"}, {"value": "-5.44E-11", "module": "D", "scenario": "S3"}]}}, {"referenceToLCIAMethodDataSet": {"shortDescription": [{"value": "Comparative toxic unit for humans (noncarcinogenic) (HTP-nc)", "lang": "en"}, {"value": "Toxizitätsvergleichseinheit für Menschen (nicht krebserregend) (HTP-nc)", "lang": "de"}], "type": "LCIA method data set", "refObjectId": "3af763a5-b7a1-48c9-9cee-1f223481fcef", "uri": "../lciamethods/3af763a5-b7a1-48c9-9cee-1f223481fcef.xml"}, "other": {"anies": [{"name": "referenceToUnitGroupDataSet", "value": {"shortDescription": [{"value": "CTUh", "lang": "en"}], "type": "unit group data set", "refObjectId": "d4c9523e-2d7e-49fd-8469-998f547d3a70", "uri": "../unitgroups/d4c9523e-2d7e-49fd-8469-998f547d3a70.xml"}}, {"value": "8.62E-08", "module": "A1-A3"}, {"value": "1.44E-09", "module": "A4"}, {"value": "8.114E-09", "module": "A5"}, {"value": "2.6E-11", "module": "B1"}, {"value": "9.46E-09", "module": "B2"}, {"value": "0", "module": "C1"}, {"value": "8.07E-11", "module": "C2"}, {"value": "2.19E-09", "module": "C3", "scenario": "S2"}, {"value": "2.48E-09", "module": "C3", "scenario": "S3"}, {"value": "7.94E-09", "module": "C4"}, {"value": "-7.78E-10", "module": "D", "scenario": "S0"}, {"value": "0", "module": "D", "scenario": "S1"}, {"value": "0", "module": "D", "scenario": "S2"}, {"value": "-3.23E-09", "module": "D", "scenario": "S3"}]}}, {"referenceToLCIAMethodDataSet": {"shortDescription": [{"value": "Soil quality index (SQP)", "lang": "en"}, {"value": "Bodenqualitätsindex (SQP)", "lang": "de"}], "type": "LCIA method data set", "refObjectId": "b2ad6890-c78d-11e6-9d9d-cec0c932ce01", "uri": "../lciamethods/b2ad6890-c78d-11e6-9d9d-cec0c932ce01.xml"}, "other": {"anies": [{"name": "referenceToUnitGroupDataSet", "value": {"shortDescription": [{"value": "SQP", "lang": "en"}], "type": "unit group data set", "refObjectId": "f130951c-e67f-4f7f-8dd4-665de3974e18", "uri": "../unitgroups/f130951c-e67f-4f7f-8dd4-665de3974e18.xml"}}, {"module": "A1-A3"}, {"module": "A4"}, {"module": "A5"}, {"module": "B1"}, {"module": "B2"}, {"module": "C1"}, {"module": "C2"}, {"module": "C3", "scenario": "S2"}, {"module": "C3", "scenario": "S3"}, {"module": "C4"}, {"module": "D", "scenario": "S0"}, {"module": "D", "scenario": "S1"}, {"module": "D", "scenario": "S2"}, {"module": "D", "scenario": "S3"}]}}]}, "otherAttributes": {"{http://www.indata.network/EPD/2019}epd-version": "1.2"}, "version": "1.1", "locations": "../ILCDLocations.xml"}