{"processInformation": {"dataSetInformation": {"UUID": "37b4961f-9a06-4ad0-8580-03033ebc1502", "name": {"baseName": [{"value": "Showerpipes", "lang": "en"}, {"value": "Duschleitungen", "lang": "de"}], "functionalUnitFlowProperties": [{"lang": "en"}]}, "classificationInformation": {"classification": [{"class": [{"value": "Gebäudetechnik", "level": 0, "classId": "8"}, {"value": "Sanitär", "level": 1, "classId": "8.3"}, {"value": "Armaturen", "level": 2, "classId": "8.3.02"}], "name": "OEKOBAU.DAT"}, {"class": [{"value": "03 Building services engineering", "level": 0}, {"value": "Sanitary facilitys", "level": 1}, {"value": "Fittings and showers", "level": 2}], "name": "IBUCategories"}]}, "generalComment": [{"value": "A showerpipe is a combination of a shower valve, shower hose and/or pipe connection and head shower and/or hand shower.\n\nShowerpipes essentially comprise of a metal housing in most cases made of brass, a plastic valve with ceramic discs or thermostatic cartridge, and several assembly parts of various materials. The pipe surface is usually chrome-plated by means of various galvanic process stages. Roughs mainly comprise of brass materials. \n\nFor the use and application of the product the respective national provisions at the place of use apply, in Germany for example the building codes of the federal states and the corresponding national specifications.\n\nThe products comply with the applicable standards and regulations listed below.", "lang": "en"}], "other": {"anies": [{"scenario": [{"description": [{"value": "Scenario 0", "lang": "en"}, {"value": "Szenario 0", "lang": "de"}], "name": "S0"}, {"description": [{"value": "100% heating of water with gas", "lang": "en"}, {"value": "100% Erwärmung von Wasser mit Gas", "lang": "de"}], "name": "S1", "default": true}, {"description": [{"value": "100% electric heating of water", "lang": "en"}, {"value": "100% elektrische Erwärmung von Wasser", "lang": "de"}], "name": "S2"}]}]}}, "quantitativeReference": {"referenceToReferenceFlow": [0]}, "time": {"referenceYear": 2023, "dataSetValidUntil": 2028, "other": {"anies": [{"name": "publicationDateOfEPD", "value": 1677196800000}]}}, "geography": {"locationOfOperationSupplyOrProduction": {"location": "GLO"}}, "technology": {"technologyDescriptionAndIncludedProcesses": [{"value": "Faucet or thermostat: No. 1: The sand core for the base body is made. No. 2: The body of the faucet is cast from brass using the sand core. No. 3: After casting, the brass body is grinded and polished. No. 4: To protect the product and make it durable, the body is galvanized with chrome. No. 5: Meanwhile, the individual parts of the cartridge are assembled. No. 6: The product parts (chrome plated brass body, cartridge, chrome plated handle and others) are lasered and assembled. No. 7: The preassembled product is packed together with the remaining components (like s-connectors and escutcheon). Overhead shower: No. 1: The plastic jet body is injected. No. 2: The plastic upper part of housing is injected. No. 3: The upper part of housing is galvanized. No. 4: The plastic thread nipple is injected. No. 5: All the parts are assembled and packed. Hand shower: No. 1: The plastic handle of the hand showers is injected. No. 2: The handle is galvanized with chrome. No. 3: The plastic inlet housing is injected. No. 4: The plastic pipe bow is injected. No. 5: The plastic distributor is injected. No. 6: Meanwhile, the plastic jet body is injected. No. 7: The distributor and the jet body are preassembled. No. 8: All the parts are assembled and packed. Hose: No. 1: The PVC inner tube is extruded. No. 2: The PVC top layer is applied on the inner tube. No. 3: The embossing foil chrome is applied on the top layer. No. 4: The hose is cut in length and assembled with the connections. Packaging: In the end all components are packed together with some additional parts like riser pipe and pipe bend. Any production waste generated is disposed accordingly. In individual cases, the production may differ slightly from the procedure (for example, if the handle is not chrome-plated). \nDeclared unit: \nThe results of this EPD are valid for the following functional unit:\n\nProvide sanitary function for one (1) average showerpipe unit used in accordance with the manufacturer's recommendations for a 20-year life, following the manufacturer's operating instructions. An average conditioned showerpipe is considered the baseline flow.\n\n Weighted averaging based on production tonnages in 2021 is chosen as basis for creating the environmental profile. 150 different showerpipes were considered.", "lang": "en"}, {"value": "Wasserhahn oder Thermostat:\n\n\nNr. 1: Der Sandkern für den Grundkörper wird hergestellt. \n\nNr. 2: Der Armaturenkörper wird unter Verwendung des Sandkerns aus Messing gegossen. \n\nNr. 3: Nach dem Gießen wird der Messingkörper geschliffen und poliert. \n\nNr. 4: Um das Produkt zu schützen und es haltbar zu machen, wird der Körper mit Chrom galvanisiert.\n\nNr. 5: In der Zwischenzeit werden die einzelnen Teile der Patrone zusammengesetzt. \n\nNr. 6: Die Produktteile (verchromter Messingkörper, Kartusche, verchromter Griff und andere) werden gelasert und montiert. \n\nNr. 7: Das vormontierte Produkt wird zusammen mit den übrigen Komponenten (wie S-Verbinder und Rosette) verpackt.\n\nKopfbrause:\n\n\nNr. 1: Der Strahlkörper aus Kunststoff wird gespritzt.\n\nNr. 2: Der obere Teil des Gehäuses aus Kunststoff wird gespritzt.\n\nNr. 3: Der obere Teil des Gehäuses ist verzinkt.\n\nNr. 4: Der Gewindenippel aus Kunststoff ist gespritzt.\n\n\nNr. 5: Alle Teile werden zusammengebaut und verpackt.\n\nHandbrause:\n\n\nNr. 1: Der Kunststoffgriff der Handbrause ist gespritzt.\n\nNr. 2: Der Griff ist verzinkt und verchromt.\n\nNr. 3: Das Einlassgehäuse aus Kunststoff ist gespritzt.\n\nNr. 4: Der Rohrbogen aus Kunststoff ist gespritzt.\n\nNr. 5: Der Kunststoffverteiler ist gespritzt.\n\nNr. 6: Der Kunststoffdüsenkörper wird gespritzt.\n\nNr. 7: Der Verteiler und der Düsenkörper werden vormontiert.\n\n\nNr. 8: Alle Teile werden zusammengebaut und verpackt.\n\nSchlauch:\n\n\nNr. 1: Das PVC-Innenrohr wird extrudiert.\n\nNr. 2: Die PVC-Deckschicht wird auf das Innenrohr aufgebracht.\n\nNr. 3: Die Chrom-Prägefolie wird auf die obere Schicht aufgebracht.\n\n\nNr. 4: Der Schlauch wird auf Länge geschnitten und mit den Anschlüssen montiert.\n\n\nVerpacken: \n\nAm Ende werden alle Komponenten zusammen mit einigen Zusatzteilen wie Steigrohr und Rohrbogen verpackt. \n\n\nAnfallende Produktionsabfälle werden entsprechend entsorgt. In Einzelfällen kann die Produktion leicht vom Verfahren abweichen (z.B. wenn der Griff nicht verchromt ist). \n", "lang": "de"}], "technologicalApplicability": [{"value": "Showerpipes are a combination of a faucet or thermostat, a overhead shower and a hand shower. Combined with hoses and riser pipe and pipe bend.\n\nThey are used in bathrooms for showering or in bathtubs.", "lang": "en"}, {"value": "Duschleitungen sind eine Kombination aus einem Wasserhahn oder Thermostat, einer Kopfbrause und einer Handbrause. Kombiniert mit Schläuchen und Steigrohren und Rohrbögen.\nSie werden in Badezimmern zum Duschen oder in Badewannen verwendet.", "lang": "de"}]}}, "modellingAndValidation": {"LCIMethodAndAllocation": {"typeOfDataSet": "EPD", "referenceToLCAMethodDetails": [{"shortDescription": [{"value": "Fittings and showers.pdf", "lang": "en"}], "type": "source data set", "refObjectId": "56798e6e-398a-4a6b-bcb4-7f7c69c74381"}], "other": {"anies": [{"name": "subType", "value": "average dataset"}]}}, "dataSourcesTreatmentAndRepresentativeness": {"referenceToDataSource": [{"shortDescription": [{"value": "GaBi Database (all versions)", "lang": "en"}], "type": "source data set", "refObjectId": "28d74cc0-db8b-4d7e-bc44-5f6d56ce0c4a"}, {"shortDescription": [{"value": "GaBi Database Edition 2021, CUP 2021.02", "lang": "en"}], "type": "source data set", "refObjectId": "90321ffe-9ebb-4946-886c-338efe6fbf26"}], "useAdviceForDataSet": [{"value": "Scope: \nThis average EPD was determined on the basis of a weighted average of production volume from 2021 and relates to the plants in Offenburg, Willstätt and Schiltach, Germany, Shanghai, China and Alpharetta, USA. This average EPD is valid for the whole product group of chrome plated showerpipes. The EPD was formed from >96% of the products involved in the sales quantity. \nSystem boundary: \nThis representative EPD follows the EPD type \"cradle to gate - with options\". The following life cycle modules are declared:\n\nModules A1-A3: \n\nThe product stage begins with considering the production of the necessary raw materials and energies, including all corresponding upstream chains and the actual procurement transports. Furthermore, the entire manufacturing phase was mapped, including the treatment of production waste until the end-of-waste status (EoW) was reached. Green electricity from hydropower is used for the manufacturing processes in Germany. US electricity mix is used for the US production site. Chinese electricity mix is used for the Chinese production site, although electricity from photovoltaic is partly used there.\n\nModule A4:\n\nAll distribution transports to the customers were considered.\n\nModule A5:\n\nThis module covers the installation process with the corresponding packaging waste generated that needs to be disposed.\n\nModules B1 & B3-B5:\n\nThese modules were considered, but evaluated as not relevant for the products and considered as zero.\n\n Module B2: \n\n Maintenance expenses are declared in this module and consist of weekly cleaning expenses for this product. \n\nModule B6:\n\n This module considers the energy input required to bring water to a certain temperature for the use of a gas low temperature boiler (scenario B6/1) and for the use of an electric instantaneous water heater (scenario B6/2).\n\n Module B7: \n\n This module considers the water consumption that can be expected depending on the function of the product family.  \n\n\nModules C1-C4:\n\nThe modules include the environmental impacts for dismantling of the products and the treatment of the waste fractions until the end-of-waste status (EoW) is reached, including the associated transports at the end of the product life cycle.\n\nModule D:\n\n\nIdentification of the benefits and costs of the product outside the system boundary. For waste, paper and plastics, these consist of energy credits from thermal utilization (A3, A5 and C3) in the form of the average European electricity mix or thermal energy from natural gas. Recycling of paper, plastic and metal scrap results in credits of the respective raw materials for the primary material portion of the input. The loads of the waste incineration and recycling processes are assigned to the respective modules (A3, A5 and C3) and not to module D.", "lang": "en"}], "other": {"anies": [{"name": "referenceToOriginalEPD", "value": {"shortDescription": {"value": "Showerpipes.pdf", "defaultValue": "Showerpipes.pdf", "lstrings": [{"lang": "en", "value": "Showerpipes.pdf"}]}, "type": "source data set", "uuid": {"uuid": "c4dfadcb-eae4-46b3-aa4d-c3a84640023f"}, "refObjectId": "c4dfadcb-eae4-46b3-aa4d-c3a84640023f", "resourceURLs": ["https://oekobaudat.de/OEKOBAU.DAT/resource/sources/c4dfadcb-eae4-46b3-aa4d-c3a84640023f/Showerpipes_14886.pdf?version=00.01.000"]}}]}}, "validation": {"review": [{"referenceToNameOfReviewerAndInstitution": [{"shortDescription": [{"value": "Institut Bauen und Umwelt e. V.", "lang": "en"}], "type": "contact data set", "refObjectId": "d111dbec-b024-4be5-86c5-752d6eb2cf95", "uri": "../contacts/d111dbec-b024-4be5-86c5-752d6eb2cf95.xml"}], "type": "Accredited third party review"}]}, "complianceDeclarations": {"compliance": [{"referenceToComplianceSystem": {"shortDescription": [{"value": "DIN EN 15804+A2", "lang": "en"}], "type": "source data set", "refObjectId": "c0016b33-8cf7-415c-ac6e-deba0d21440d", "uri": "../sources/c0016b33-8cf7-415c-ac6e-deba0d21440d.xml"}}, {"referenceToComplianceSystem": {"shortDescription": [{"value": "ISO 14025", "lang": "en"}], "type": "source data set", "refObjectId": "4f2eb655-6e44-4874-a95a-e28f5442cd4d", "uri": "../sources/4f2eb655-6e44-4874-a95a-e28f5442cd4d.xml"}}]}}, "administrativeInformation": {"commissionerAndGoal": {"referenceToCommissioner": [{"shortDescription": [{"value": "Hansgrohe Group", "lang": "en"}], "type": "contact data set", "refObjectId": "e2e7bc1a-4fae-4c47-9754-a0a4995bdebe", "uri": "../contacts/e2e7bc1a-4fae-4c47-9754-a0a4995bdebe.xml"}]}, "dataGenerator": {"referenceToPersonOrEntityGeneratingTheDataSet": [{"shortDescription": [{"value": "brands and values GmbH", "lang": "en"}], "type": "contact data set", "refObjectId": "6b539b8a-10e3-4004-8ccc-a79f169aa339", "uri": "../contacts/6b539b8a-10e3-4004-8ccc-a79f169aa339.xml"}]}, "dataEntryBy": {"timeStamp": 1677239039173, "referenceToDataSetFormat": [{"shortDescription": [{"value": "ILCD Format", "lang": "en"}], "type": "source data set", "refObjectId": "a97a0155-0234-4b87-b4ce-a45da52f2a40", "uri": "../sources/a97a0155-0234-4b87-b4ce-a45da52f2a40.xml"}, {"shortDescription": [{"value": "EPD-Datenformaterweiterungen v1.2", "lang": "de"}, {"value": "EPD Data Format Extensions v1.2", "lang": "en"}], "type": "source data set", "refObjectId": "a29449fd-aa2f-4de8-b5d7-4b06b43c6fde", "uri": "../sources/a29449fd-aa2f-4de8-b5d7-4b06b43c6fde.xml"}]}, "publicationAndOwnership": {"dataSetVersion": "00.01.000", "referenceToRegistrationAuthority": {"shortDescription": [{"value": "Institut Bauen und Umwelt e. V.", "lang": "en"}], "type": "contact data set", "refObjectId": "d111dbec-b024-4be5-86c5-752d6eb2cf95", "uri": "../contacts/d111dbec-b024-4be5-86c5-752d6eb2cf95.xml"}, "registrationNumber": "EPD-HAN-20230022-ICC1-EN", "referenceToOwnershipOfDataSet": {"shortDescription": [{"value": "Hansgrohe Group", "lang": "en"}], "type": "contact data set", "refObjectId": "e2e7bc1a-4fae-4c47-9754-a0a4995bdebe", "uri": "../contacts/e2e7bc1a-4fae-4c47-9754-a0a4995bdebe.xml"}, "copyright": true, "licenseType": "Free of charge for all users and uses", "accessRestrictions": [{"value": "None", "lang": "en"}], "other": {"anies": [{"name": "referenceToPublisher", "value": {"shortDescription": [{"value": "Institut Bauen und Umwelt e. V.", "lang": "en"}], "type": "contact data set", "refObjectId": "d111dbec-b024-4be5-86c5-752d6eb2cf95", "uri": "../contacts/d111dbec-b024-4be5-86c5-752d6eb2cf95.xml"}}]}}}, "exchanges": {"exchange": [{"dataSetInternalID": 0, "referenceToFlowDataSet": {"shortDescription": [{"value": "Showerpipe ()", "lang": "en"}], "type": "flow data set", "refObjectId": "08fa9b2e-5db2-4ea4-a130-d15c35ecda41", "uri": "../flows/08fa9b2e-5db2-4ea4-a130-d15c35ecda41.xml"}, "meanAmount": 1.0, "referencesToDataSource": {}, "referenceFlow": true, "resolvedFlowVersion": "00.01.000", "resultingflowAmount": 1.0, "flowProperties": [{"name": [{"lang": "en", "value": "Number of pieces"}, {"lang": "de", "value": "Anzahl"}], "uuid": "01846770-4cfe-4a25-8ad9-919d8d378345", "referenceFlowProperty": true, "meanValue": 1.0, "referenceUnit": "pcs.", "unitGroupUUID": "934110e3-baf4-49e9-992c-3d8109a6aafb"}], "materialProperties": [{"name": "mass reference", "value": "6.734", "unit": "kg/m^3", "unitDescription": "Kilogram per cubic meter "}], "typeOfFlow": "Product flow", "classification": {"classHierarchy": "Gebäudetechnik / Sanitär / Armaturen", "name": "OEKOBAU.DAT"}}, {"dataSetInternalID": 1, "referenceToFlowDataSet": {"shortDescription": [{"value": "Renewable primary energy as energy carrier (PERE)", "lang": "en"}, {"value": "Erneuerbare Primärenergie als Energieträger (PERE)", "lang": "de"}], "type": "flow data set", "refObjectId": "20f32be5-0398-4288-9b6d-accddd195317", "uri": "../flows/20f32be5-0398-4288-9b6d-accddd195317.xml"}, "exchange direction": "INPUT", "other": {"anies": [{"name": "referenceToUnitGroupDataSet", "value": {"shortDescription": [{"value": "MJ", "lang": "en"}], "type": "unit group data set", "refObjectId": "93a60a57-a3c8-11da-a746-0800200c9a66", "uri": "../unitgroups/93a60a57-a3c8-11da-a746-0800200c9a66.xml"}}, {"value": "30.2960183674553", "module": "A1-A3"}, {"value": "0.27", "module": "A4"}, {"value": "33.5339816325447", "module": "A5"}, {"value": "0", "module": "B1"}, {"value": "93.6", "module": "B2"}, {"value": "0", "module": "B3"}, {"value": "0", "module": "B4"}, {"value": "0", "module": "B5"}, {"value": "179", "module": "B6", "scenario": "S1"}, {"value": "14600", "module": "B6", "scenario": "S2"}, {"value": "172", "module": "B7"}, {"value": "0", "module": "C1"}, {"value": "0.0634", "module": "C2"}, {"value": "0.992", "module": "C3"}, {"value": "0.0137", "module": "C4"}, {"value": "-58.5", "module": "D"}]}, "resolvedFlowVersion": "38.00.000", "flowProperties": [], "typeOfFlow": "Other flow", "classification": {"classHierarchy": "Quantities", "name": "GaBiCategories"}}, {"dataSetInternalID": 2, "referenceToFlowDataSet": {"shortDescription": [{"value": "Renewable primary energy resources as material utilization (PERM)", "lang": "en"}, {"value": "Erneuerbare Primärenergie zur stofflichen Nutzung (PERM)", "lang": "de"}], "type": "flow data set", "refObjectId": "fb3ec0de-548d-4508-aea5-00b73bf6f702", "uri": "../flows/fb3ec0de-548d-4508-aea5-00b73bf6f702.xml"}, "exchange direction": "INPUT", "other": {"anies": [{"name": "referenceToUnitGroupDataSet", "value": {"shortDescription": [{"value": "MJ", "lang": "en"}], "type": "unit group data set", "refObjectId": "93a60a57-a3c8-11da-a746-0800200c9a66", "uri": "../unitgroups/93a60a57-a3c8-11da-a746-0800200c9a66.xml"}}, {"value": "31.5039816325447", "module": "A1-A3"}, {"value": "0", "module": "A4"}, {"value": "-31.5039816325447", "module": "A5"}, {"value": "0", "module": "B1"}, {"value": "0", "module": "B2"}, {"value": "0", "module": "B3"}, {"value": "0", "module": "B4"}, {"value": "0", "module": "B5"}, {"value": "-1", "module": "B6", "scenario": "S1"}, {"value": "0", "module": "B6", "scenario": "S2"}, {"value": "0", "module": "B7"}, {"value": "0", "module": "C1"}, {"value": "0", "module": "C2"}, {"value": "0", "module": "C3"}, {"value": "0", "module": "C4"}, {"value": "0", "module": "D"}]}, "resolvedFlowVersion": "38.00.000", "flowProperties": [], "typeOfFlow": "Other flow", "classification": {"classHierarchy": "Quantities", "name": "GaBiCategories"}}, {"dataSetInternalID": 3, "referenceToFlowDataSet": {"shortDescription": [{"value": "Total use of renewable primary energy resources (PERT)", "lang": "en"}, {"value": "Total erneuerbare Primärenergie (PERT)", "lang": "de"}], "type": "flow data set", "refObjectId": "53f97275-fa8a-4cdd-9024-65936002acd0", "uri": "../flows/53f97275-fa8a-4cdd-9024-65936002acd0.xml"}, "exchange direction": "INPUT", "other": {"anies": [{"name": "referenceToUnitGroupDataSet", "value": {"shortDescription": [{"value": "MJ", "lang": "en"}], "type": "unit group data set", "refObjectId": "93a60a57-a3c8-11da-a746-0800200c9a66", "uri": "../unitgroups/93a60a57-a3c8-11da-a746-0800200c9a66.xml"}}, {"value": "61.8", "module": "A1-A3"}, {"value": "0.27", "module": "A4"}, {"value": "2.03", "module": "A5"}, {"value": "0", "module": "B1"}, {"value": "93.6", "module": "B2"}, {"value": "0", "module": "B3"}, {"value": "0", "module": "B4"}, {"value": "0", "module": "B5"}, {"value": "178", "module": "B6", "scenario": "S1"}, {"value": "14600", "module": "B6", "scenario": "S2"}, {"value": "172", "module": "B7"}, {"value": "0", "module": "C1"}, {"value": "0.0634", "module": "C2"}, {"value": "0.992", "module": "C3"}, {"value": "0.0137", "module": "C4"}, {"value": "-58.5", "module": "D"}]}, "resolvedFlowVersion": "38.00.000", "flowProperties": [], "typeOfFlow": "Other flow", "classification": {"classHierarchy": "Quantities / Environmental quantities / EPD EN 15804 / LCI indicators", "name": "GaBiCategories"}}, {"dataSetInternalID": 4, "referenceToFlowDataSet": {"shortDescription": [{"value": "Non renewable primary energy as energy carrier (PENRE)", "lang": "en"}, {"value": "Nicht-erneuerbare Primärenergie als Energieträger (PENRE)", "lang": "de"}], "type": "flow data set", "refObjectId": "ac857178-2b45-46ec-892a-a9a4332f0372", "uri": "../flows/ac857178-2b45-46ec-892a-a9a4332f0372.xml"}, "exchange direction": "INPUT", "other": {"anies": [{"name": "referenceToUnitGroupDataSet", "value": {"shortDescription": [{"value": "MJ", "lang": "en"}], "type": "unit group data set", "refObjectId": "93a60a57-a3c8-11da-a746-0800200c9a66", "uri": "../unitgroups/93a60a57-a3c8-11da-a746-0800200c9a66.xml"}}, {"value": "248.539730463579", "module": "A1-A3"}, {"value": "5.81", "module": "A4"}, {"value": "7.82336276509146", "module": "A5"}, {"value": "0", "module": "B1"}, {"value": "452", "module": "B2"}, {"value": "0", "module": "B3"}, {"value": "0", "module": "B4"}, {"value": "0", "module": "B5"}, {"value": "20501", "module": "B6", "scenario": "S1"}, {"value": "31600", "module": "B6", "scenario": "S2"}, {"value": "586", "module": "B7"}, {"value": "0", "module": "C1"}, {"value": "1.11", "module": "C2"}, {"value": "27.6195614327629", "module": "C3"}, {"value": "1.49534533856647", "module": "C4"}, {"value": "-87.4", "module": "D"}]}, "resolvedFlowVersion": "38.00.000", "flowProperties": [], "typeOfFlow": "Other flow", "classification": {"classHierarchy": "Quantities", "name": "GaBiCategories"}}, {"dataSetInternalID": 5, "referenceToFlowDataSet": {"shortDescription": [{"value": "Non renewable primary energy as material utilization (PENRM)", "lang": "en"}, {"value": "Nicht-erneuerbare Primärenergie zur stofflichen Nutzung (PENRM)", "lang": "de"}], "type": "flow data set", "refObjectId": "1421caa0-679d-4bf4-b282-0eb850ccae27", "uri": "../flows/1421caa0-679d-4bf4-b282-0eb850ccae27.xml"}, "exchange direction": "INPUT", "other": {"anies": [{"name": "referenceToUnitGroupDataSet", "value": {"shortDescription": [{"value": "MJ", "lang": "en"}], "type": "unit group data set", "refObjectId": "93a60a57-a3c8-11da-a746-0800200c9a66", "uri": "../unitgroups/93a60a57-a3c8-11da-a746-0800200c9a66.xml"}}, {"value": "28.4602695364208", "module": "A1-A3"}, {"value": "0", "module": "A4"}, {"value": "-2.31336276509146", "module": "A5"}, {"value": "0", "module": "B1"}, {"value": "0", "module": "B2"}, {"value": "0", "module": "B3"}, {"value": "0", "module": "B4"}, {"value": "0", "module": "B5"}, {"value": "-1", "module": "B6", "scenario": "S1"}, {"value": "0", "module": "B6", "scenario": "S2"}, {"value": "0", "module": "B7"}, {"value": "0", "module": "C1"}, {"value": "0", "module": "C2"}, {"value": "-24.8395614327629", "module": "C3"}, {"value": "-1.30734533856647", "module": "C4"}, {"value": "0", "module": "D"}]}, "resolvedFlowVersion": "38.00.000", "flowProperties": [], "typeOfFlow": "Other flow", "classification": {"classHierarchy": "Quantities", "name": "GaBiCategories"}}, {"dataSetInternalID": 6, "referenceToFlowDataSet": {"shortDescription": [{"value": "Total use of non renewable primary energy resources (PENRT)", "lang": "en"}, {"value": "Total nicht erneuerbare Primärenergie (PENRT)", "lang": "de"}], "type": "flow data set", "refObjectId": "06159210-646b-4c8d-8583-da9b3b95a6c1", "uri": "../flows/06159210-646b-4c8d-8583-da9b3b95a6c1.xml"}, "exchange direction": "INPUT", "other": {"anies": [{"name": "referenceToUnitGroupDataSet", "value": {"shortDescription": [{"value": "MJ", "lang": "en"}], "type": "unit group data set", "refObjectId": "93a60a57-a3c8-11da-a746-0800200c9a66", "uri": "../unitgroups/93a60a57-a3c8-11da-a746-0800200c9a66.xml"}}, {"value": "277", "module": "A1-A3"}, {"value": "5.81", "module": "A4"}, {"value": "5.51", "module": "A5"}, {"value": "0", "module": "B1"}, {"value": "452", "module": "B2"}, {"value": "0", "module": "B3"}, {"value": "0", "module": "B4"}, {"value": "0", "module": "B5"}, {"value": "20500", "module": "B6", "scenario": "S1"}, {"value": "31600", "module": "B6", "scenario": "S2"}, {"value": "586", "module": "B7"}, {"value": "0", "module": "C1"}, {"value": "1.11", "module": "C2"}, {"value": "2.78", "module": "C3"}, {"value": "0.188", "module": "C4"}, {"value": "-87.4", "module": "D"}]}, "resolvedFlowVersion": "38.00.000", "flowProperties": [], "typeOfFlow": "Other flow", "classification": {"classHierarchy": "Quantities / Environmental quantities / EPD EN 15804 / LCI indicators", "name": "GaBiCategories"}}, {"dataSetInternalID": 7, "referenceToFlowDataSet": {"shortDescription": [{"value": "Use of secondary material (SM)", "lang": "en"}, {"value": "Einsatz von Sekundärstoffen (SM)", "lang": "de"}], "type": "flow data set", "refObjectId": "c6a1f35f-2d09-4f54-8dfb-97e502e1ce92", "uri": "../flows/c6a1f35f-2d09-4f54-8dfb-97e502e1ce92.xml"}, "exchange direction": "INPUT", "other": {"anies": [{"name": "referenceToUnitGroupDataSet", "value": {"shortDescription": [{"value": "kg", "lang": "en"}], "type": "unit group data set", "refObjectId": "ad38d542-3fe9-439d-9b95-2f5f7752acaf", "uri": "../unitgroups/ad38d542-3fe9-439d-9b95-2f5f7752acaf.xml"}}, {"value": "2.26", "module": "A1-A3"}, {"value": "0", "module": "A4"}, {"value": "0", "module": "A5"}, {"value": "0", "module": "B1"}, {"value": "0", "module": "B2"}, {"value": "0", "module": "B3"}, {"value": "0", "module": "B4"}, {"value": "0", "module": "B5"}, {"value": "0", "module": "B6", "scenario": "S1"}, {"value": "0", "module": "B6", "scenario": "S2"}, {"value": "0", "module": "B7"}, {"value": "0", "module": "C1"}, {"value": "0", "module": "C2"}, {"value": "0", "module": "C3"}, {"value": "0", "module": "C4"}, {"value": "3.03", "module": "D"}]}, "resolvedFlowVersion": "38.00.000", "flowProperties": [], "typeOfFlow": "Other flow", "classification": {"classHierarchy": "Quantities / Environmental quantities / EPD EN 15804 / LCI indicators", "name": "GaBiCategories"}}, {"dataSetInternalID": 8, "referenceToFlowDataSet": {"shortDescription": [{"value": "Use of renewable secondary fuels (RSF)", "lang": "en"}, {"value": "Erneuerbare Sekundärbrennstoffe (RSF)", "lang": "de"}], "type": "flow data set", "refObjectId": "64333088-a55f-4aa2-9a31-c10b07816787", "uri": "../flows/64333088-a55f-4aa2-9a31-c10b07816787.xml"}, "exchange direction": "INPUT", "other": {"anies": [{"name": "referenceToUnitGroupDataSet", "value": {"shortDescription": [{"value": "MJ", "lang": "en"}], "type": "unit group data set", "refObjectId": "93a60a57-a3c8-11da-a746-0800200c9a66", "uri": "../unitgroups/93a60a57-a3c8-11da-a746-0800200c9a66.xml"}}, {"value": "4.12E-23", "module": "A1-A3"}, {"value": "0", "module": "A4"}, {"value": "0", "module": "A5"}, {"value": "0", "module": "B1"}, {"value": "0", "module": "B2"}, {"value": "0", "module": "B3"}, {"value": "0", "module": "B4"}, {"value": "0", "module": "B5"}, {"value": "0", "module": "B6", "scenario": "S1"}, {"value": "0", "module": "B6", "scenario": "S2"}, {"value": "0", "module": "B7"}, {"value": "0", "module": "C1"}, {"value": "0", "module": "C2"}, {"value": "0", "module": "C3"}, {"value": "0", "module": "C4"}, {"value": "-8.59E-23", "module": "D"}]}, "resolvedFlowVersion": "38.00.000", "flowProperties": [], "typeOfFlow": "Other flow", "classification": {"classHierarchy": "Quantities / Environmental quantities / EPD EN 15804 / LCI indicators", "name": "GaBiCategories"}}, {"dataSetInternalID": 9, "referenceToFlowDataSet": {"shortDescription": [{"value": "Use of non renewable secondary fuels (NRSF)", "lang": "en"}, {"value": "Nicht erneuerbare Sekundärbrennstoffe (NRSF)", "lang": "de"}], "type": "flow data set", "refObjectId": "89def144-d39a-4287-b86f-efde453ddcb2", "uri": "../flows/89def144-d39a-4287-b86f-efde453ddcb2.xml"}, "exchange direction": "INPUT", "other": {"anies": [{"name": "referenceToUnitGroupDataSet", "value": {"shortDescription": [{"value": "MJ", "lang": "en"}], "type": "unit group data set", "refObjectId": "93a60a57-a3c8-11da-a746-0800200c9a66", "uri": "../unitgroups/93a60a57-a3c8-11da-a746-0800200c9a66.xml"}}, {"value": "0", "module": "A1-A3"}, {"value": "0", "module": "A4"}, {"value": "0", "module": "A5"}, {"value": "0", "module": "B1"}, {"value": "0", "module": "B2"}, {"value": "0", "module": "B3"}, {"value": "0", "module": "B4"}, {"value": "0", "module": "B5"}, {"value": "0", "module": "B6", "scenario": "S1"}, {"value": "0", "module": "B6", "scenario": "S2"}, {"value": "0", "module": "B7"}, {"value": "0", "module": "C1"}, {"value": "0", "module": "C2"}, {"value": "0", "module": "C3"}, {"value": "0", "module": "C4"}, {"value": "0", "module": "D"}]}, "resolvedFlowVersion": "38.00.000", "flowProperties": [], "typeOfFlow": "Other flow", "classification": {"classHierarchy": "Quantities / Environmental quantities / EPD EN 15804 / LCI indicators", "name": "GaBiCategories"}}, {"dataSetInternalID": 10, "referenceToFlowDataSet": {"shortDescription": [{"value": "Use of net fresh water (FW)", "lang": "en"}, {"value": "Einsatz von Süßwasserressourcen (FW)", "lang": "de"}], "type": "flow data set", "refObjectId": "3cf952c8-f3a4-461d-8c96-96456ca62246", "uri": "../flows/3cf952c8-f3a4-461d-8c96-96456ca62246.xml"}, "exchange direction": "INPUT", "other": {"anies": [{"name": "referenceToUnitGroupDataSet", "value": {"shortDescription": [{"value": "m^3", "lang": "en"}], "type": "unit group data set", "refObjectId": "cd950537-0a98-4044-9ba7-9f9a68d0a504", "uri": "../unitgroups/cd950537-0a98-4044-9ba7-9f9a68d0a504.xml"}}, {"value": "0.516", "module": "A1-A3"}, {"value": "0.000311", "module": "A4"}, {"value": "0.00372", "module": "A5"}, {"value": "0", "module": "B1"}, {"value": "0.162", "module": "B2"}, {"value": "0", "module": "B3"}, {"value": "0", "module": "B4"}, {"value": "0", "module": "B5"}, {"value": "0.2", "module": "B6", "scenario": "S1"}, {"value": "14.2", "module": "B6", "scenario": "S2"}, {"value": "0.499", "module": "B7"}, {"value": "0", "module": "C1"}, {"value": "7.26E-05", "module": "C2"}, {"value": "0.00695", "module": "C3"}, {"value": "2.25E-06", "module": "C4"}, {"value": "-0.36", "module": "D"}]}, "resolvedFlowVersion": "38.00.000", "flowProperties": [], "typeOfFlow": "Other flow", "classification": {"classHierarchy": "Quantities / Environmental quantities / EPD EN 15804 / LCI indicators", "name": "GaBiCategories"}}, {"dataSetInternalID": 11, "referenceToFlowDataSet": {"shortDescription": [{"value": "Hazardous waste disposed (HWD)", "lang": "en"}, {"value": "Gefährlicher Abfall zur Deponie (HWD)", "lang": "de"}], "type": "flow data set", "refObjectId": "430f9e0f-59b2-46a0-8e0d-55e0e84948fc", "uri": "../flows/430f9e0f-59b2-46a0-8e0d-55e0e84948fc.xml"}, "exchange direction": "OUTPUT", "other": {"anies": [{"name": "referenceToUnitGroupDataSet", "value": {"shortDescription": [{"value": "kg", "lang": "en"}], "type": "unit group data set", "refObjectId": "ad38d542-3fe9-439d-9b95-2f5f7752acaf", "uri": "../unitgroups/ad38d542-3fe9-439d-9b95-2f5f7752acaf.xml"}}, {"value": "1.15E-05", "module": "A1-A3"}, {"value": "2.54E-10", "module": "A4"}, {"value": "3.78E-09", "module": "A5"}, {"value": "0", "module": "B1"}, {"value": "0.0085", "module": "B2"}, {"value": "0", "module": "B3"}, {"value": "0", "module": "B4"}, {"value": "0", "module": "B5"}, {"value": "3.83E-06", "module": "B6", "scenario": "S1"}, {"value": "8.35E-06", "module": "B6", "scenario": "S2"}, {"value": "1.2E-07", "module": "B7"}, {"value": "0", "module": "C1"}, {"value": "5.82E-11", "module": "C2"}, {"value": "6.57E-10", "module": "C3"}, {"value": "3.34E-11", "module": "C4"}, {"value": "-5.19E-05", "module": "D"}]}, "resolvedFlowVersion": "38.00.000", "flowProperties": [], "typeOfFlow": "Other flow", "classification": {"classHierarchy": "Quantities / Environmental quantities / EPD EN 15804 / LCI indicators", "name": "GaBiCategories"}}, {"dataSetInternalID": 12, "referenceToFlowDataSet": {"shortDescription": [{"value": "Non hazardous waste disposed (NHWD)", "lang": "en"}, {"value": "Entsorgter nicht gefährlicher Abfall (NHWD)", "lang": "de"}], "type": "flow data set", "refObjectId": "b29ef66b-e286-4afa-949f-62f1a7b4d7fa", "uri": "../flows/b29ef66b-e286-4afa-949f-62f1a7b4d7fa.xml"}, "exchange direction": "OUTPUT", "other": {"anies": [{"name": "referenceToUnitGroupDataSet", "value": {"shortDescription": [{"value": "kg", "lang": "en"}], "type": "unit group data set", "refObjectId": "ad38d542-3fe9-439d-9b95-2f5f7752acaf", "uri": "../unitgroups/ad38d542-3fe9-439d-9b95-2f5f7752acaf.xml"}}, {"value": "2.7", "module": "A1-A3"}, {"value": "0.000845", "module": "A4"}, {"value": "0.0636", "module": "A5"}, {"value": "0", "module": "B1"}, {"value": "0.658", "module": "B2"}, {"value": "0", "module": "B3"}, {"value": "0", "module": "B4"}, {"value": "0", "module": "B5"}, {"value": "2.69", "module": "B6", "scenario": "S1"}, {"value": "22.4", "module": "B6", "scenario": "S2"}, {"value": "93.5", "module": "B7"}, {"value": "0", "module": "C1"}, {"value": "0.000173", "module": "C2"}, {"value": "0.154", "module": "C3"}, {"value": "0.244", "module": "C4"}, {"value": "-1.87", "module": "D"}]}, "resolvedFlowVersion": "38.00.000", "flowProperties": [], "typeOfFlow": "Other flow", "classification": {"classHierarchy": "Quantities / Environmental quantities / EPD EN 15804 / LCI indicators", "name": "GaBiCategories"}}, {"dataSetInternalID": 13, "referenceToFlowDataSet": {"shortDescription": [{"value": "Radioactive waste disposed (RWD)", "lang": "en"}, {"value": "Entsorgter radioaktiver Abfall (RWD)", "lang": "de"}], "type": "flow data set", "refObjectId": "3449546e-52ad-4b39-b809-9fb77cea8ff6", "uri": "../flows/3449546e-52ad-4b39-b809-9fb77cea8ff6.xml"}, "exchange direction": "OUTPUT", "other": {"anies": [{"name": "referenceToUnitGroupDataSet", "value": {"shortDescription": [{"value": "kg", "lang": "en"}], "type": "unit group data set", "refObjectId": "ad38d542-3fe9-439d-9b95-2f5f7752acaf", "uri": "../unitgroups/ad38d542-3fe9-439d-9b95-2f5f7752acaf.xml"}}, {"value": "0.00739", "module": "A1-A3"}, {"value": "9.72E-06", "module": "A4"}, {"value": "0.000234", "module": "A5"}, {"value": "0", "module": "B1"}, {"value": "0.00413", "module": "B2"}, {"value": "0", "module": "B3"}, {"value": "0", "module": "B4"}, {"value": "0", "module": "B5"}, {"value": "0.0452", "module": "B6", "scenario": "S1"}, {"value": "4.71", "module": "B6", "scenario": "S2"}, {"value": "0.0481", "module": "B7"}, {"value": "0", "module": "C1"}, {"value": "2.01E-06", "module": "C2"}, {"value": "0.000145", "module": "C3"}, {"value": "2.16E-06", "module": "C4"}, {"value": "-0.00328", "module": "D"}]}, "resolvedFlowVersion": "38.00.000", "flowProperties": [], "typeOfFlow": "Other flow", "classification": {"classHierarchy": "Quantities / Environmental quantities / EPD EN 15804 / LCI indicators", "name": "GaBiCategories"}}, {"dataSetInternalID": 14, "referenceToFlowDataSet": {"shortDescription": [{"value": "Components for re-use (CRU)", "lang": "en"}, {"value": "Komponenten für die Wiederverwendung (CRU)", "lang": "de"}], "type": "flow data set", "refObjectId": "a2b32f97-3fc7-4af2-b209-525bc6426f33", "uri": "../flows/a2b32f97-3fc7-4af2-b209-525bc6426f33.xml"}, "exchange direction": "OUTPUT", "other": {"anies": [{"name": "referenceToUnitGroupDataSet", "value": {"shortDescription": [{"value": "kg", "lang": "en"}], "type": "unit group data set", "refObjectId": "ad38d542-3fe9-439d-9b95-2f5f7752acaf", "uri": "../unitgroups/ad38d542-3fe9-439d-9b95-2f5f7752acaf.xml"}}, {"value": "0", "module": "A1-A3"}, {"value": "0", "module": "A4"}, {"value": "0", "module": "A5"}, {"value": "0", "module": "B1"}, {"value": "0", "module": "B2"}, {"value": "0", "module": "B3"}, {"value": "0", "module": "B4"}, {"value": "0", "module": "B5"}, {"value": "0", "module": "B6", "scenario": "S1"}, {"value": "0", "module": "B6", "scenario": "S2"}, {"value": "0", "module": "B7"}, {"value": "0", "module": "C1"}, {"value": "0", "module": "C2"}, {"value": "0", "module": "C3"}, {"value": "0", "module": "C4"}, {"value": "0", "module": "D"}]}, "resolvedFlowVersion": "38.00.000", "flowProperties": [], "typeOfFlow": "Other flow", "classification": {"classHierarchy": "Quantities / Environmental quantities / EPD EN 15804 / LCI indicators", "name": "GaBiCategories"}}, {"dataSetInternalID": 15, "referenceToFlowDataSet": {"shortDescription": [{"value": "Materials for recycling (MFR)", "lang": "en"}, {"value": "Stoffe zum Recycling (MFR)", "lang": "de"}], "type": "flow data set", "refObjectId": "d7fe48a5-4103-49c8-9aae-b0b5dfdbd6ae", "uri": "../flows/d7fe48a5-4103-49c8-9aae-b0b5dfdbd6ae.xml"}, "exchange direction": "OUTPUT", "other": {"anies": [{"name": "referenceToUnitGroupDataSet", "value": {"shortDescription": [{"value": "kg", "lang": "en"}], "type": "unit group data set", "refObjectId": "ad38d542-3fe9-439d-9b95-2f5f7752acaf", "uri": "../unitgroups/ad38d542-3fe9-439d-9b95-2f5f7752acaf.xml"}}, {"value": "0", "module": "A1-A3"}, {"value": "0", "module": "A4"}, {"value": "1.67", "module": "A5"}, {"value": "0", "module": "B1"}, {"value": "0", "module": "B2"}, {"value": "0", "module": "B3"}, {"value": "0", "module": "B4"}, {"value": "0", "module": "B5"}, {"value": "0", "module": "B6", "scenario": "S1"}, {"value": "0", "module": "B6", "scenario": "S2"}, {"value": "0", "module": "B7"}, {"value": "0", "module": "C1"}, {"value": "0", "module": "C2"}, {"value": "3.29", "module": "C3"}, {"value": "0", "module": "C4"}, {"value": "0", "module": "D"}]}, "resolvedFlowVersion": "38.00.000", "flowProperties": [], "typeOfFlow": "Other flow", "classification": {"classHierarchy": "Quantities / Environmental quantities / EPD EN 15804 / LCI indicators", "name": "GaBiCategories"}}, {"dataSetInternalID": 16, "referenceToFlowDataSet": {"shortDescription": [{"value": "Materials for energy recovery (MER)", "lang": "en"}, {"value": "Stoffe für die Energierückgewinnung (MER)", "lang": "de"}], "type": "flow data set", "refObjectId": "59a9181c-3aaf-46ee-8b13-2b3723b6e447", "uri": "../flows/59a9181c-3aaf-46ee-8b13-2b3723b6e447.xml"}, "exchange direction": "OUTPUT", "other": {"anies": [{"name": "referenceToUnitGroupDataSet", "value": {"shortDescription": [{"value": "kg", "lang": "en"}], "type": "unit group data set", "refObjectId": "ad38d542-3fe9-439d-9b95-2f5f7752acaf", "uri": "../unitgroups/ad38d542-3fe9-439d-9b95-2f5f7752acaf.xml"}}, {"value": "0", "module": "A1-A3"}, {"value": "0", "module": "A4"}, {"value": "0", "module": "A5"}, {"value": "0", "module": "B1"}, {"value": "0", "module": "B2"}, {"value": "0", "module": "B3"}, {"value": "0", "module": "B4"}, {"value": "0", "module": "B5"}, {"value": "0", "module": "B6", "scenario": "S1"}, {"value": "0", "module": "B6", "scenario": "S2"}, {"value": "0", "module": "B7"}, {"value": "0", "module": "C1"}, {"value": "0", "module": "C2"}, {"value": "0", "module": "C3"}, {"value": "0", "module": "C4"}, {"value": "0", "module": "D"}]}, "resolvedFlowVersion": "38.00.000", "flowProperties": [], "typeOfFlow": "Other flow", "classification": {"classHierarchy": "Quantities / Environmental quantities / EPD EN 15804 / LCI indicators", "name": "GaBiCategories"}}, {"dataSetInternalID": 17, "referenceToFlowDataSet": {"shortDescription": [{"value": "Exported electrical energy (EEE)", "lang": "en"}, {"value": "Exportierte elektrische Energie (EEE)", "lang": "de"}], "type": "flow data set", "refObjectId": "4da0c987-2b76-40d6-9e9e-82a017aaaf29", "uri": "../flows/4da0c987-2b76-40d6-9e9e-82a017aaaf29.xml"}, "exchange direction": "OUTPUT", "other": {"anies": [{"name": "referenceToUnitGroupDataSet", "value": {"shortDescription": [{"value": "MJ", "lang": "en"}], "type": "unit group data set", "refObjectId": "93a60a57-a3c8-11da-a746-0800200c9a66", "uri": "../unitgroups/93a60a57-a3c8-11da-a746-0800200c9a66.xml"}}, {"value": "0.285", "module": "A1-A3"}, {"value": "0", "module": "A4"}, {"value": "0.52", "module": "A5"}, {"value": "0", "module": "B1"}, {"value": "0", "module": "B2"}, {"value": "0", "module": "B3"}, {"value": "0", "module": "B4"}, {"value": "0", "module": "B5"}, {"value": "0", "module": "B6", "scenario": "S1"}, {"value": "0", "module": "B6", "scenario": "S2"}, {"value": "0", "module": "B7"}, {"value": "0", "module": "C1"}, {"value": "0", "module": "C2"}, {"value": "0.0288", "module": "C3"}, {"value": "0.00029", "module": "C4"}, {"value": "0", "module": "D"}]}, "resolvedFlowVersion": "38.00.000", "flowProperties": [], "typeOfFlow": "Other flow", "classification": {"classHierarchy": "Quantities / Environmental quantities / EPD EN 15804 / LCI indicators", "name": "GaBiCategories"}}, {"dataSetInternalID": 18, "referenceToFlowDataSet": {"shortDescription": [{"value": "Exported thermal energy (EET)", "lang": "en"}, {"value": "Exportierte thermische Energie (EET)", "lang": "de"}], "type": "flow data set", "refObjectId": "98daf38a-7a79-46d3-9a37-2b7bd0955810", "uri": "../flows/98daf38a-7a79-46d3-9a37-2b7bd0955810.xml"}, "exchange direction": "OUTPUT", "other": {"anies": [{"name": "referenceToUnitGroupDataSet", "value": {"shortDescription": [{"value": "MJ", "lang": "en"}], "type": "unit group data set", "refObjectId": "93a60a57-a3c8-11da-a746-0800200c9a66", "uri": "../unitgroups/93a60a57-a3c8-11da-a746-0800200c9a66.xml"}}, {"value": "0.616", "module": "A1-A3"}, {"value": "0", "module": "A4"}, {"value": "0.938", "module": "A5"}, {"value": "0", "module": "B1"}, {"value": "0", "module": "B2"}, {"value": "0", "module": "B3"}, {"value": "0", "module": "B4"}, {"value": "0", "module": "B5"}, {"value": "0", "module": "B6", "scenario": "S1"}, {"value": "0", "module": "B6", "scenario": "S2"}, {"value": "0", "module": "B7"}, {"value": "0", "module": "C1"}, {"value": "0", "module": "C2"}, {"value": "0.0541", "module": "C3"}, {"value": "0", "module": "C4"}, {"value": "0", "module": "D"}]}, "resolvedFlowVersion": "38.00.000", "flowProperties": [], "typeOfFlow": "Other flow", "classification": {"classHierarchy": "Quantities / Environmental quantities / EPD EN 15804 / LCI indicators", "name": "GaBiCategories"}}]}, "LCIAResults": {"LCIAResult": [{"referenceToLCIAMethodDataSet": {"shortDescription": [{"value": "Global Warming Potential total (GWP-total)", "lang": "en"}, {"value": "Globales Erwärmungspotenzial total (GWP-total)", "lang": "de"}], "type": "LCIA method data set", "refObjectId": "6a37f984-a4b3-458a-a20a-64418c145fa2", "uri": "../lciamethods/6a37f984-a4b3-458a-a20a-64418c145fa2.xml"}, "other": {"anies": [{"name": "referenceToUnitGroupDataSet", "value": {"shortDescription": [{"value": "kg CO_(2)-Äq.", "lang": "en"}], "type": "unit group data set", "refObjectId": "1ebf3012-d0db-4de2-aefd-ef30cedb0be1", "uri": "../unitgroups/1ebf3012-d0db-4de2-aefd-ef30cedb0be1.xml"}}, {"value": "15.9882", "module": "A1-A3"}, {"value": "0.44484", "module": "A4"}, {"value": "2.677692", "module": "A5"}, {"value": "0", "module": "B1"}, {"value": "25.62", "module": "B2"}, {"value": "0", "module": "B3"}, {"value": "0", "module": "B4"}, {"value": "0", "module": "B5"}, {"value": "1190.0604", "module": "B6", "scenario": "S1"}, {"value": "1782.51", "module": "B6", "scenario": "S2"}, {"value": "56.946", "module": "B7"}, {"value": "0", "module": "C1"}, {"value": "0.083076", "module": "C2"}, {"value": "2.660365", "module": "C3"}, {"value": "0.0130125", "module": "C4"}, {"value": "-9.53817879523415", "module": "D"}]}}, {"referenceToLCIAMethodDataSet": {"shortDescription": [{"value": "Global Warming Potential fossil fuels (GWP-fossil)", "lang": "en"}, {"value": "Globales Erwärmungspotenzial fossil (GWP-fossil)", "lang": "de"}], "type": "LCIA method data set", "refObjectId": "5f635281-343e-44fb-83df-1971b155e6b6", "uri": "../lciamethods/5f635281-343e-44fb-83df-1971b155e6b6.xml"}, "other": {"anies": [{"name": "referenceToUnitGroupDataSet", "value": {"shortDescription": [{"value": "kg CO_(2)-Äq.", "lang": "en"}], "type": "unit group data set", "refObjectId": "1ebf3012-d0db-4de2-aefd-ef30cedb0be1", "uri": "../unitgroups/1ebf3012-d0db-4de2-aefd-ef30cedb0be1.xml"}}, {"value": "18.2", "module": "A1-A3"}, {"value": "0.442", "module": "A4"}, {"value": "0.427", "module": "A5"}, {"value": "0", "module": "B1"}, {"value": "19.6", "module": "B2"}, {"value": "0", "module": "B3"}, {"value": "0", "module": "B4"}, {"value": "0", "module": "B5"}, {"value": "1190", "module": "B6", "scenario": "S1"}, {"value": "1780", "module": "B6", "scenario": "S2"}, {"value": "56.9", "module": "B7"}, {"value": "0", "module": "C1"}, {"value": "0.0824", "module": "C2"}, {"value": "2.66", "module": "C3"}, {"value": "0.013", "module": "C4"}, {"value": "-7.39", "module": "D"}]}}, {"referenceToLCIAMethodDataSet": {"shortDescription": [{"value": "Global Warming Potential biogenic (GWP-biogenic)", "lang": "en"}, {"value": "Globales Erwärmungspotenzial biogen (GWP-biogenic)", "lang": "de"}], "type": "LCIA method data set", "refObjectId": "2356e1ab-0185-4db5-86e5-16de51c7485c", "uri": "../lciamethods/2356e1ab-0185-4db5-86e5-16de51c7485c.xml"}, "other": {"anies": [{"name": "referenceToUnitGroupDataSet", "value": {"shortDescription": [{"value": "kg CO_(2)-Äq.", "lang": "en"}], "type": "unit group data set", "refObjectId": "1ebf3012-d0db-4de2-aefd-ef30cedb0be1", "uri": "../unitgroups/1ebf3012-d0db-4de2-aefd-ef30cedb0be1.xml"}}, {"value": "-2.25", "module": "A1-A3"}, {"value": "0", "module": "A4"}, {"value": "2.25", "module": "A5"}, {"value": "0", "module": "B1"}, {"value": "0", "module": "B2"}, {"value": "0", "module": "B3"}, {"value": "0", "module": "B4"}, {"value": "0", "module": "B5"}, {"value": "0", "module": "B6", "scenario": "S1"}, {"value": "0", "module": "B6", "scenario": "S2"}, {"value": "0", "module": "B7"}, {"value": "0", "module": "C1"}, {"value": "0", "module": "C2"}, {"value": "0", "module": "C3"}, {"value": "0", "module": "C4"}, {"value": "-2.12557879523415", "module": "D"}]}}, {"referenceToLCIAMethodDataSet": {"shortDescription": [{"value": "Global Warming Potential luluc (GWP-luluc)", "lang": "en"}, {"value": "Globales Erwärmungspotenzial luluc (GWP-luluc)", "lang": "de"}], "type": "LCIA method data set", "refObjectId": "4331bbdb-978a-490d-8707-eeb047f01a55", "uri": "../lciamethods/4331bbdb-978a-490d-8707-eeb047f01a55.xml"}, "other": {"anies": [{"name": "referenceToUnitGroupDataSet", "value": {"shortDescription": [{"value": "kg CO_(2)-Äq.", "lang": "en"}], "type": "unit group data set", "refObjectId": "1ebf3012-d0db-4de2-aefd-ef30cedb0be1", "uri": "../unitgroups/1ebf3012-d0db-4de2-aefd-ef30cedb0be1.xml"}}, {"value": "0.0382", "module": "A1-A3"}, {"value": "0.00284", "module": "A4"}, {"value": "0.000692", "module": "A5"}, {"value": "0", "module": "B1"}, {"value": "6.02", "module": "B2"}, {"value": "0", "module": "B3"}, {"value": "0", "module": "B4"}, {"value": "0", "module": "B5"}, {"value": "0.0604", "module": "B6", "scenario": "S1"}, {"value": "2.51", "module": "B6", "scenario": "S2"}, {"value": "0.046", "module": "B7"}, {"value": "0", "module": "C1"}, {"value": "0.000676", "module": "C2"}, {"value": "0.000365", "module": "C3"}, {"value": "1.25E-05", "module": "C4"}, {"value": "-0.0226", "module": "D"}]}}, {"referenceToLCIAMethodDataSet": {"shortDescription": [{"value": "Depletion potential of the stratospheric ozone layer (ODP)", "lang": "en"}, {"value": "Abbau Potential der stratosphärischen Ozonschicht (ODP)", "lang": "de"}], "type": "LCIA method data set", "refObjectId": "b5c629d6-def3-11e6-bf01-fe55135034f3", "uri": "../lciamethods/b5c629d6-def3-11e6-bf01-fe55135034f3.xml"}, "other": {"anies": [{"name": "referenceToUnitGroupDataSet", "value": {"shortDescription": [{"value": "kg CFC11-Äq.", "lang": "en"}], "type": "unit group data set", "refObjectId": "d9e957c9-7309-4474-bf3a-7777df6c4e5b", "uri": "../unitgroups/d9e957c9-7309-4474-bf3a-7777df6c4e5b.xml"}}, {"value": "5.24E-08", "module": "A1-A3"}, {"value": "7.84E-17", "module": "A4"}, {"value": "3.12E-15", "module": "A5"}, {"value": "0", "module": "B1"}, {"value": "1.09E-06", "module": "B2"}, {"value": "0", "module": "B3"}, {"value": "0", "module": "B4"}, {"value": "0", "module": "B5"}, {"value": "4.3E-13", "module": "B6", "scenario": "S1"}, {"value": "4.25E-11", "module": "B6", "scenario": "S2"}, {"value": "5.38E-13", "module": "B7"}, {"value": "0", "module": "C1"}, {"value": "1.63E-17", "module": "C2"}, {"value": "7.42E-10", "module": "C3"}, {"value": "3.09E-17", "module": "C4"}, {"value": "-9.65E-08", "module": "D"}]}}, {"referenceToLCIAMethodDataSet": {"shortDescription": [{"value": "Acidification potential of land and water (AP)", "lang": "en"}, {"value": "Versauerungspotenzial von Boden und Wasser (AP)", "lang": "de"}], "type": "LCIA method data set", "refObjectId": "b5c611c6-def3-11e6-bf01-fe55135034f3", "uri": "../lciamethods/b5c611c6-def3-11e6-bf01-fe55135034f3.xml"}, "other": {"anies": [{"name": "referenceToUnitGroupDataSet", "value": {"shortDescription": [{"value": "mol H^(+)-Äq.", "lang": "en"}], "type": "unit group data set", "refObjectId": "42e089ac-92bf-4bf2-8ca1-5fc40d18f2ed", "uri": "../unitgroups/42e089ac-92bf-4bf2-8ca1-5fc40d18f2ed.xml"}}, {"value": "0.183", "module": "A1-A3"}, {"value": "0.00412", "module": "A4"}, {"value": "0.00115", "module": "A5"}, {"value": "0", "module": "B1"}, {"value": "0.0664", "module": "B2"}, {"value": "0", "module": "B3"}, {"value": "0", "module": "B4"}, {"value": "0", "module": "B5"}, {"value": "0.732", "module": "B6", "scenario": "S1"}, {"value": "3.7", "module": "B6", "scenario": "S2"}, {"value": "0.14", "module": "B7"}, {"value": "0", "module": "C1"}, {"value": "0.000138", "module": "C2"}, {"value": "0.000967", "module": "C3"}, {"value": "4.09E-05", "module": "C4"}, {"value": "-0.0864", "module": "D"}]}}, {"referenceToLCIAMethodDataSet": {"shortDescription": [{"value": "Eutrophication potential aquatic freshwater (EP-freshwater)", "lang": "en"}, {"value": "Eutrophierungspotenzial Süßwasser (EP-freshwater)", "lang": "de"}], "type": "LCIA method data set", "refObjectId": "b53ec18f-7377-4ad3-86eb-cc3f4f276b2b", "uri": "../lciamethods/b53ec18f-7377-4ad3-86eb-cc3f4f276b2b.xml"}, "other": {"anies": [{"name": "referenceToUnitGroupDataSet", "value": {"shortDescription": [{"value": "kg PO_(4)-Äq.", "lang": "en"}], "type": "unit group data set", "refObjectId": "0429039d-a61d-4590-ba67-aa4a20a810a1", "uri": "../unitgroups/0429039d-a61d-4590-ba67-aa4a20a810a1.xml"}}, {"value": "0.00106", "module": "A1-A3"}, {"value": "1.05E-06", "module": "A4"}, {"value": "7.49E-07", "module": "A5"}, {"value": "0", "module": "B1"}, {"value": "0.000581", "module": "B2"}, {"value": "0", "module": "B3"}, {"value": "0", "module": "B4"}, {"value": "0", "module": "B5"}, {"value": "0.000109", "module": "B6", "scenario": "S1"}, {"value": "0.00476", "module": "B6", "scenario": "S2"}, {"value": "0.0605", "module": "B7"}, {"value": "0", "module": "C1"}, {"value": "2.46E-07", "module": "C2"}, {"value": "5.29E-07", "module": "C3"}, {"value": "7.45E-07", "module": "C4"}, {"value": "-0.000736", "module": "D"}]}}, {"referenceToLCIAMethodDataSet": {"shortDescription": [{"value": "Eutrophication potential aquatic marine (EP-marine)", "lang": "en"}, {"value": "Eutrophierungspotenzial Salzwasser (EP-marine)", "lang": "de"}], "type": "LCIA method data set", "refObjectId": "b5c619fa-def3-11e6-bf01-fe55135034f3", "uri": "../lciamethods/b5c619fa-def3-11e6-bf01-fe55135034f3.xml"}, "other": {"anies": [{"name": "referenceToUnitGroupDataSet", "value": {"shortDescription": [{"value": "kg N-Äq.", "lang": "en"}], "type": "unit group data set", "refObjectId": "d05bb823-ecdf-4686-8c40-bf1d9257859f", "uri": "../unitgroups/d05bb823-ecdf-4686-8c40-bf1d9257859f.xml"}}, {"value": "0.0222", "module": "A1-A3"}, {"value": "0.00116", "module": "A4"}, {"value": "0.000252", "module": "A5"}, {"value": "0", "module": "B1"}, {"value": "0.0151", "module": "B2"}, {"value": "0", "module": "B3"}, {"value": "0", "module": "B4"}, {"value": "0", "module": "B5"}, {"value": "0.311", "module": "B6", "scenario": "S1"}, {"value": "0.878", "module": "B6", "scenario": "S2"}, {"value": "0.265", "module": "B7"}, {"value": "0", "module": "C1"}, {"value": "5.44E-05", "module": "C2"}, {"value": "0.000373", "module": "C3"}, {"value": "1.01E-05", "module": "C4"}, {"value": "-0.0104", "module": "D"}]}}, {"referenceToLCIAMethodDataSet": {"shortDescription": [{"value": "Eutrophication potential terrestrial (EP-terrestrial)", "lang": "en"}, {"value": "Eutrophierungspotenzial Land (EP-terrestrial)", "lang": "de"}], "type": "LCIA method data set", "refObjectId": "b5c614d2-def3-11e6-bf01-fe55135034f3", "uri": "../lciamethods/b5c614d2-def3-11e6-bf01-fe55135034f3.xml"}, "other": {"anies": [{"name": "referenceToUnitGroupDataSet", "value": {"shortDescription": [{"value": "mol N-Äq.", "lang": "en"}], "type": "unit group data set", "refObjectId": "71b4d617-0ec9-4d3f-b65e-e438940c2401", "uri": "../unitgroups/71b4d617-0ec9-4d3f-b65e-e438940c2401.xml"}}, {"value": "0.235", "module": "A1-A3"}, {"value": "0.0129", "module": "A4"}, {"value": "0.0028", "module": "A5"}, {"value": "0", "module": "B1"}, {"value": "0.181", "module": "B2"}, {"value": "0", "module": "B3"}, {"value": "0", "module": "B4"}, {"value": "0", "module": "B5"}, {"value": "3.4", "module": "B6", "scenario": "S1"}, {"value": "9.22", "module": "B6", "scenario": "S2"}, {"value": "0.418", "module": "B7"}, {"value": "0", "module": "C1"}, {"value": "0.000622", "module": "C2"}, {"value": "0.00452", "module": "C3"}, {"value": "0.000109", "module": "C4"}, {"value": "-0.111", "module": "D"}]}}, {"referenceToLCIAMethodDataSet": {"shortDescription": [{"value": "Formation potential of tropospheric ozone photochemical oxidants (POCP)", "lang": "en"}, {"value": "Bildungspotential für troposphärisches Ozon (POCP)", "lang": "de"}], "type": "LCIA method data set", "refObjectId": "b5c610fe-def3-11e6-bf01-fe55135034f3", "uri": "../lciamethods/b5c610fe-def3-11e6-bf01-fe55135034f3.xml"}, "other": {"anies": [{"name": "referenceToUnitGroupDataSet", "value": {"shortDescription": [{"value": "kg NMVOC-Äq.", "lang": "en"}], "type": "unit group data set", "refObjectId": "d27c25f8-fbc1-44c6-b47b-4adbae4199c6", "uri": "../unitgroups/d27c25f8-fbc1-44c6-b47b-4adbae4199c6.xml"}}, {"value": "0.0648", "module": "A1-A3"}, {"value": "0.00313", "module": "A4"}, {"value": "0.000809", "module": "A5"}, {"value": "0", "module": "B1"}, {"value": "0.0604", "module": "B2"}, {"value": "0", "module": "B3"}, {"value": "0", "module": "B4"}, {"value": "0", "module": "B5"}, {"value": "0.908", "module": "B6", "scenario": "S1"}, {"value": "2.38", "module": "B6", "scenario": "S2"}, {"value": "0.107", "module": "B7"}, {"value": "0", "module": "C1"}, {"value": "0.000123", "module": "C2"}, {"value": "0.000989", "module": "C3"}, {"value": "3.17E-05", "module": "C4"}, {"value": "-0.031", "module": "D"}]}}, {"referenceToLCIAMethodDataSet": {"shortDescription": [{"value": "Abiotic depletion potential for non fossil resources (ADPE)", "lang": "en"}, {"value": "Potenzial für den abiotischen Abbau nicht fossiler Ressourcen (ADPE)", "lang": "de"}], "type": "LCIA method data set", "refObjectId": "b2ad6494-c78d-11e6-9d9d-cec0c932ce01", "uri": "../lciamethods/b2ad6494-c78d-11e6-9d9d-cec0c932ce01.xml"}, "other": {"anies": [{"name": "referenceToUnitGroupDataSet", "value": {"shortDescription": [{"value": "kg Sb-Äq.", "lang": "en"}], "type": "unit group data set", "refObjectId": "54ccd2d9-a32a-4fc2-923d-f2c8c93e89d4", "uri": "../unitgroups/54ccd2d9-a32a-4fc2-923d-f2c8c93e89d4.xml"}}, {"value": "0.00669", "module": "A1-A3"}, {"value": "3.37E-08", "module": "A4"}, {"value": "5.67E-06", "module": "A5"}, {"value": "0", "module": "B1"}, {"value": "2.11E-05", "module": "B2"}, {"value": "0", "module": "B3"}, {"value": "0", "module": "B4"}, {"value": "0", "module": "B5"}, {"value": "6.41E-05", "module": "B6", "scenario": "S1"}, {"value": "0.000523", "module": "B6", "scenario": "S2"}, {"value": "7.41E-06", "module": "B7"}, {"value": "0", "module": "C1"}, {"value": "7.33E-09", "module": "C2"}, {"value": "5.06E-08", "module": "C3"}, {"value": "8.94E-10", "module": "C4"}, {"value": "-0.00525", "module": "D"}]}}, {"referenceToLCIAMethodDataSet": {"shortDescription": [{"value": "Abiotic depletion potential for fossil resources (ADPF)", "lang": "en"}, {"value": "Potenzial für den abiotischen Abbau fossiler Brennstoffe (ADPF)", "lang": "de"}], "type": "LCIA method data set", "refObjectId": "b2ad6110-c78d-11e6-9d9d-cec0c932ce01", "uri": "../lciamethods/b2ad6110-c78d-11e6-9d9d-cec0c932ce01.xml"}, "other": {"anies": [{"name": "referenceToUnitGroupDataSet", "value": {"shortDescription": [{"value": "MJ", "lang": "en"}], "type": "unit group data set", "refObjectId": "93a60a57-a3c8-11da-a746-0800200c9a66", "uri": "../unitgroups/93a60a57-a3c8-11da-a746-0800200c9a66.xml"}}, {"value": "277", "module": "A1-A3"}, {"value": "5.79", "module": "A4"}, {"value": "5.51", "module": "A5"}, {"value": "0", "module": "B1"}, {"value": "452", "module": "B2"}, {"value": "0", "module": "B3"}, {"value": "0", "module": "B4"}, {"value": "0", "module": "B5"}, {"value": "20500", "module": "B6", "scenario": "S1"}, {"value": "31600", "module": "B6", "scenario": "S2"}, {"value": "585", "module": "B7"}, {"value": "0", "module": "C1"}, {"value": "1.1", "module": "C2"}, {"value": "2.78", "module": "C3"}, {"value": "0.188", "module": "C4"}, {"value": "-87.1", "module": "D"}]}}, {"referenceToLCIAMethodDataSet": {"shortDescription": [{"value": "Water use (WDP)", "lang": "en"}, {"value": "Wassernutzung (WDP)", "lang": "de"}], "type": "LCIA method data set", "refObjectId": "b2ad66ce-c78d-11e6-9d9d-cec0c932ce01", "uri": "../lciamethods/b2ad66ce-c78d-11e6-9d9d-cec0c932ce01.xml"}, "other": {"anies": [{"name": "referenceToUnitGroupDataSet", "value": {"shortDescription": [{"value": "m^(3) world-Äq. deprived", "lang": "en"}], "type": "unit group data set", "refObjectId": "6ae2df01-888e-46c8-b17d-49fa3869b476", "uri": "../unitgroups/6ae2df01-888e-46c8-b17d-49fa3869b476.xml"}}, {"value": "21.2", "module": "A1-A3"}, {"value": "0.00337", "module": "A4"}, {"value": "0.115", "module": "A5"}, {"value": "0", "module": "B1"}, {"value": "6.93", "module": "B2"}, {"value": "0", "module": "B3"}, {"value": "0", "module": "B4"}, {"value": "0", "module": "B5"}, {"value": "3.13", "module": "B6", "scenario": "S1"}, {"value": "285", "module": "B6", "scenario": "S2"}, {"value": "17.5", "module": "B7"}, {"value": "0", "module": "C1"}, {"value": "0.000767", "module": "C2"}, {"value": "0.279", "module": "C3"}, {"value": "-0.000141", "module": "C4"}, {"value": "-15.7", "module": "D"}]}}, {"referenceToLCIAMethodDataSet": {"shortDescription": [{"value": "Incidence of disease due to PM emissions (PM)", "lang": "en"}, {"value": "Auftreten von Krankheiten aufgrund von Feinstaubemissionen (PM)", "lang": "de"}], "type": "LCIA method data set", "refObjectId": "b5c602c6-def3-11e6-bf01-fe55135034f3", "uri": "../lciamethods/b5c602c6-def3-11e6-bf01-fe55135034f3.xml"}, "other": {"anies": [{"name": "referenceToUnitGroupDataSet", "value": {"shortDescription": [{"value": "Disease incidence", "lang": "en"}], "type": "unit group data set", "refObjectId": "3883559b-648f-4afc-8ba2-0bd24f3affa3", "uri": "../unitgroups/3883559b-648f-4afc-8ba2-0bd24f3affa3.xml"}}, {"value": "1.67E-06", "module": "A1-A3"}, {"value": "6.41E-08", "module": "A4"}, {"value": "1.31E-08", "module": "A5"}, {"value": "0", "module": "B1"}, {"value": "3.31E-06", "module": "B2"}, {"value": "0", "module": "B3"}, {"value": "0", "module": "B4"}, {"value": "0", "module": "B5"}, {"value": "5.08E-06", "module": "B6", "scenario": "S1"}, {"value": "3.12E-05", "module": "B6", "scenario": "S2"}, {"value": "1.57E-06", "module": "B7"}, {"value": "0", "module": "C1"}, {"value": "8.64E-10", "module": "C2"}, {"value": "9E-09", "module": "C3"}, {"value": "4.33E-10", "module": "C4"}, {"value": "-8.96E-07", "module": "D"}]}}, {"referenceToLCIAMethodDataSet": {"shortDescription": [{"value": "Human exposure efficiency relative to U235 (IR)", "lang": "en"}, {"value": "Wirkung durch Exposition des Menschen mit U235 (IR)", "lang": "de"}], "type": "LCIA method data set", "refObjectId": "b5c632be-def3-11e6-bf01-fe55135034f3", "uri": "../lciamethods/b5c632be-def3-11e6-bf01-fe55135034f3.xml"}, "other": {"anies": [{"name": "referenceToUnitGroupDataSet", "value": {"shortDescription": [{"value": "kBq U235-Äq.", "lang": "en"}], "type": "unit group data set", "refObjectId": "456b05bf-1415-44a9-9993-02452f554c09", "uri": "../unitgroups/456b05bf-1415-44a9-9993-02452f554c09.xml"}}, {"value": "3.37", "module": "A1-A3"}, {"value": "0.00142", "module": "A4"}, {"value": "0.0352", "module": "A5"}, {"value": "0", "module": "B1"}, {"value": "2.14", "module": "B2"}, {"value": "0", "module": "B3"}, {"value": "0", "module": "B4"}, {"value": "0", "module": "B5"}, {"value": "7.19", "module": "B6", "scenario": "S1"}, {"value": "772", "module": "B6", "scenario": "S2"}, {"value": "7.57", "module": "B7"}, {"value": "0", "module": "C1"}, {"value": "0.000293", "module": "C2"}, {"value": "0.0141", "module": "C3"}, {"value": "0.000309", "module": "C4"}, {"value": "-1.92", "module": "D"}]}}, {"referenceToLCIAMethodDataSet": {"shortDescription": [{"value": "Comparative toxic unit for ecosystems (ETP-fw)", "lang": "en"}, {"value": "Toxizitätsvergleichseinheit für Ökosysteme (ETP-fw)", "lang": "de"}], "type": "LCIA method data set", "refObjectId": "ee1082d1-b0f7-43ca-a1f0-21e2a4a74511", "uri": "../lciamethods/ee1082d1-b0f7-43ca-a1f0-21e2a4a74511.xml"}, "other": {"anies": [{"name": "referenceToUnitGroupDataSet", "value": {"shortDescription": [{"value": "CTUe", "lang": "en"}], "type": "unit group data set", "refObjectId": "aa959ded-f1eb-4efb-9c5c-2d60be36b3e6", "uri": "../unitgroups/aa959ded-f1eb-4efb-9c5c-2d60be36b3e6.xml"}}, {"value": "1420", "module": "A1-A3"}, {"value": "4.27", "module": "A4"}, {"value": "2.18", "module": "A5"}, {"value": "0", "module": "B1"}, {"value": "200", "module": "B2"}, {"value": "0", "module": "B3"}, {"value": "0", "module": "B4"}, {"value": "0", "module": "B5"}, {"value": "280", "module": "B6", "scenario": "S1"}, {"value": "13300", "module": "B6", "scenario": "S2"}, {"value": "8260", "module": "B7"}, {"value": "0", "module": "C1"}, {"value": "0.817", "module": "C2"}, {"value": "2.48", "module": "C3"}, {"value": "0.0938", "module": "C4"}, {"value": "-166", "module": "D"}]}}, {"referenceToLCIAMethodDataSet": {"shortDescription": [{"value": "Comparative toxic unit for humans (carcinogenic) (HTP-c)", "lang": "en"}, {"value": "Toxizitätsvergleichseinheit für Menschen (krebserregend) (HTP-c)", "lang": "de"}], "type": "LCIA method data set", "refObjectId": "2299222a-bbd8-474f-9d4f-4dd1f18aea7c", "uri": "../lciamethods/2299222a-bbd8-474f-9d4f-4dd1f18aea7c.xml"}, "other": {"anies": [{"name": "referenceToUnitGroupDataSet", "value": {"shortDescription": [{"value": "CTUh", "lang": "en"}], "type": "unit group data set", "refObjectId": "d4c9523e-2d7e-49fd-8469-998f547d3a70", "uri": "../unitgroups/d4c9523e-2d7e-49fd-8469-998f547d3a70.xml"}}, {"value": "4.39E-07", "module": "A1-A3"}, {"value": "8.51E-11", "module": "A4"}, {"value": "1.66E-08", "module": "A5"}, {"value": "0", "module": "B1"}, {"value": "2.21E-08", "module": "B2"}, {"value": "0", "module": "B3"}, {"value": "0", "module": "B4"}, {"value": "0", "module": "B5"}, {"value": "5.99E-08", "module": "B6", "scenario": "S1"}, {"value": "3.76E-07", "module": "B6", "scenario": "S2"}, {"value": "2.81E-07", "module": "B7"}, {"value": "0", "module": "C1"}, {"value": "1.65E-11", "module": "C2"}, {"value": "7E-11", "module": "C3"}, {"value": "6.99E-12", "module": "C4"}, {"value": "-1.92E-08", "module": "D"}]}}, {"referenceToLCIAMethodDataSet": {"shortDescription": [{"value": "Comparative toxic unit for humans (noncarcinogenic) (HTP-nc)", "lang": "en"}, {"value": "Toxizitätsvergleichseinheit für Menschen (nicht krebserregend) (HTP-nc)", "lang": "de"}], "type": "LCIA method data set", "refObjectId": "3af763a5-b7a1-48c9-9cee-1f223481fcef", "uri": "../lciamethods/3af763a5-b7a1-48c9-9cee-1f223481fcef.xml"}, "other": {"anies": [{"name": "referenceToUnitGroupDataSet", "value": {"shortDescription": [{"value": "CTUh", "lang": "en"}], "type": "unit group data set", "refObjectId": "d4c9523e-2d7e-49fd-8469-998f547d3a70", "uri": "../unitgroups/d4c9523e-2d7e-49fd-8469-998f547d3a70.xml"}}, {"value": "1.96E-06", "module": "A1-A3"}, {"value": "4.42E-09", "module": "A4"}, {"value": "1.28E-07", "module": "A5"}, {"value": "0", "module": "B1"}, {"value": "7.49E-07", "module": "B2"}, {"value": "0", "module": "B3"}, {"value": "0", "module": "B4"}, {"value": "0", "module": "B5"}, {"value": "6.32E-06", "module": "B6", "scenario": "S1"}, {"value": "1.42E-05", "module": "B6", "scenario": "S2"}, {"value": "2.89E-05", "module": "B7"}, {"value": "0", "module": "C1"}, {"value": "8.79E-10", "module": "C2"}, {"value": "6.33E-09", "module": "C3"}, {"value": "6.63E-10", "module": "C4"}, {"value": "-5.28E-07", "module": "D"}]}}, {"referenceToLCIAMethodDataSet": {"shortDescription": [{"value": "Soil quality index (SQP)", "lang": "en"}, {"value": "Bodenqualitätsindex (SQP)", "lang": "de"}], "type": "LCIA method data set", "refObjectId": "b2ad6890-c78d-11e6-9d9d-cec0c932ce01", "uri": "../lciamethods/b2ad6890-c78d-11e6-9d9d-cec0c932ce01.xml"}, "other": {"anies": [{"name": "referenceToUnitGroupDataSet", "value": {"shortDescription": [{"value": "SQP", "lang": "en"}], "type": "unit group data set", "refObjectId": "f130951c-e67f-4f7f-8dd4-665de3974e18", "uri": "../unitgroups/f130951c-e67f-4f7f-8dd4-665de3974e18.xml"}}, {"value": "109", "module": "A1-A3"}, {"value": "1.59", "module": "A4"}, {"value": "7.4", "module": "A5"}, {"value": "0", "module": "B1"}, {"value": "318", "module": "B2"}, {"value": "0", "module": "B3"}, {"value": "0", "module": "B4"}, {"value": "0", "module": "B5"}, {"value": "119", "module": "B6", "scenario": "S1"}, {"value": "9970", "module": "B6", "scenario": "S2"}, {"value": "289", "module": "B7"}, {"value": "0", "module": "C1"}, {"value": "0.379", "module": "C2"}, {"value": "0.865", "module": "C3"}, {"value": "0.0137", "module": "C4"}, {"value": "-273", "module": "D"}]}}]}, "otherAttributes": {"{http://www.indata.network/EPD/2019}epd-version": "1.2"}, "version": "1.1", "locations": "../ILCDLocations.xml"}