{"processInformation": {"dataSetInformation": {"UUID": "37beb0f7-d72f-4a59-a55c-4e0e1b579efe", "name": {"baseName": [{"value": "Kooltherm® K3 / Kooltherm® K10", "lang": "en"}, {"value": "Kooltherm® K3", "lang": "de"}], "functionalUnitFlowProperties": [{"lang": "en"}]}, "classificationInformation": {"classification": [{"class": [{"value": "Dämmstoffe", "level": 0, "classId": "2"}, {"value": "Phenolharz-Hartschaum (PF)", "level": 1, "classId": "2.5"}, {"value": "PF-Platten", "level": 2, "classId": "2.5.01"}], "name": "OEKOBAU.DAT"}, {"class": [{"value": "02 Building products", "level": 0}, {"value": "Thermal insulation products", "level": 1}, {"value": "Insulating materials made of foam plastics", "level": 2}], "name": "IBUCategories"}]}, "generalComment": [{"value": "Kooltherm® K3 / Kooltherm® K10 is a rigid thermoset cellular insulation material faced on both sides with a glass tissue based facing. The product is available in variable thicknesses from 20 mm up to 160 mm. This EPD is based on a thickness of 80 mm and RD-value of 3,80 m·K/W.", "lang": "en"}, {"value": "Kooltherm® K3 ist ein steifes, duroplastisches, zelluläres Isoliermaterial, das beidseitig mit einer Deckschicht auf Glasgewebebasis versehen ist. Das Produkt ist in variablen Dicken von 20 mm bis 160 mm erhältlich. Diese EPD basiert auf einer Dicke von 80 mm und einem RD-Wert von 3,80 m²-K/W.", "lang": "de"}]}, "quantitativeReference": {"referenceToReferenceFlow": [0]}, "time": {"referenceYear": 2023, "dataSetValidUntil": 2028, "other": {"anies": [{"name": "publicationDateOfEPD", "value": 1695340800000}]}}, "geography": {"locationOfOperationSupplyOrProduction": {"location": "RER"}}, "technology": {"technologyDescriptionAndIncludedProcesses": [{"value": "Phenolic foam is produced by the use of phenolic resin, a catalyst, additives and blowing agent. The cell structure is formed in the resin under the influence of heat released during the chemical reaction. Hereby, the blowing agent is incorporated into the material which forms a solid and very fine cell structure, which is nearly 100% closed. The foam is applied on the glass fiber facings. After this, the thickness and strength is determined by the conveyor belt where upper and lower rollers compress the material into the desired thickness. The board is sawed into the correct size and packed according to the product specification. Declared unit:The declared unit (1m²) and conversion factors are listed in the table below. \nTechnical data: \nThe declaration of performance of the product can be found at www.kingspan.com. \nDeclared unit: \nThe declared unit (1 m) and conversion factors are listed in the table below.", "lang": "en"}, {"value": "Phenolschaum wird durch die Verwendung von Phenolharz, einem Katalysator, Additiven und einem Treibmittel hergestellt. Die Zellstruktur wird im Harz unter dem Einfluss der bei der chemischen Reaktion freigesetzten Wärme gebildet. Dabei wird das Treibmittel in das Material eingearbeitet, das eine feste und sehr feine Zellstruktur bildet, die zu fast 100% geschlossen ist. Der Schaum wird auf die Glasfaserbeläge aufgetragen. Danach wird die Dicke und Stärke durch das Förderband bestimmt, auf dem obere und untere Walzen das Material auf die gewünschte Dicke komprimieren. Die Platte wird auf die richtige Größe gesägt und entsprechend der Produktspezifikation verpackt.\n\nDeklarierte Einheit: Die deklarierte Einheit (1m²) und die Umrechnungsfaktoren sind in der untenstehenden Tabelle aufgeführt. \nTechnische Daten: \nDie Leistungserklärung des Produkts finden Sie unter www.kingspan.com. \nDeklarierte Einheit: \nDie angegebene Einheit (1 m²) und die Umrechnungsfaktoren sind in der nachstehenden Tabelle aufgeführt.", "lang": "de"}], "technologicalApplicability": [{"value": "Kooltherm® K3 is suitable for use as floor insulation.\nKooltherm® K10 is suitable for use as soffit insulation.", "lang": "en"}, {"value": "Kooltherm® K3 ist für die Verwendung als Bodendämmung geeignet.", "lang": "de"}]}}, "modellingAndValidation": {"LCIMethodAndAllocation": {"typeOfDataSet": "EPD", "referenceToLCAMethodDetails": [{"shortDescription": [{"value": "Insulating materials made of foam plastics.pdf", "lang": "en"}], "type": "source data set", "refObjectId": "61ce7b2b-122b-49f7-aa0d-8228a7f7753d"}], "other": {"anies": [{"name": "subType", "value": "specific dataset"}]}}, "dataSourcesTreatmentAndRepresentativeness": {"referenceToDataSource": [{"shortDescription": [{"value": "GaBi Database (all versions)", "lang": "en"}], "type": "source data set", "refObjectId": "28d74cc0-db8b-4d7e-bc44-5f6d56ce0c4a"}, {"shortDescription": [{"value": "GaBi Database Edition 2022, CUP 2022.02", "lang": "en"}], "type": "source data set", "refObjectId": "94f442cb-662e-43ea-a792-4b0a35132e93"}], "useAdviceForDataSet": [{"value": "Scope: \nThe insulation material Kooltherm® K3 / Kooltherm® K10 is produced by Kingspan Insulation B.V. at the manufacturing facilities in Tiel, the Netherlands and Jnkping, Sweden. This EPD is based on weighted averages which have been determined on the basis of the single values originating from the different Kingspan Insulation factories. \n\nKooltherm® K3 / Kooltherm® K10 is a rigid thermoset cellular insulation material faced on both sides with a glass tissue based facing.\n\nIn order to enable the user of the EPD to calculate the LCA results for different thicknesses, the EPD contains the respective calculation rules. \nSystem boundary: \nThe type of EPD according to EN 15804 is: cradle to gate with options, modules C1–C4, and module D (A1–A3, C, D and additional modules:A4, A5). \n\nThe product stage is a mandatory information module and it covers: \n· A1, raw material extraction and processing, processing of secondary material input (e.g. recycling processes), \n· A2, transport to the manufacturer, \n· A3, manufacturing, including provision of all materials, products and energy, packaging processing and its transport, as well as waste processing up to the end-of-waste state or disposal of final residues during the product stage.\n\nThe construction process stage includes: \n· A4 transport to the building site; \n· A5 installation in the building including provision of all materials, products and energy, as well as waste processing up to the end-of-waste state or disposal of final residues during the construction process stage.\nThe end-of-life stage is a mandatory information module and it covers: \n· C1 de-construction, demolition; \n· C2 transport to waste processing; \n· C3 waste processing for reuse, recovery and/or recycling; \n· C4 disposal (not applicable for this EPD) including provision and all transport, provision of all materials, products and related energy and water use. \n\nEnvironmental burden of the incineration (R1 > 60 %) of the product at the end-of-life stage are assigned to the product system(C3); resulting potential credits for thermal and electrical energy from energy substitution are declared in module D.\n\n\nFactors for different thicknesses\nThe LCA results for the insulation material declared in this EPD refer to a product with a thickness of 80 mm. To enable the user of the EPD to calculate the results for different thicknesses the factors in the following table can be used for the calculation. The LCA results in chapter 5 have to be multiplied by these factors. The scaling factors are applicable for the complete product, where the facings are for all product thicknesses equal, and the foam inputs are scaling upwards and downwards with other product thicknesses.\n\nBackground data from GaBi ts Version 10 is used with GaBi data sets CUP2022.1", "lang": "en"}, {"value": "Gültigkeitsbereich: \nDer Dämmstoff Kooltherm® K3 wird von Kingspan Insulation B.V. in den Produktionsstätten in Tiel, Niederlande, und Jönköping, Schweden, hergestellt. Diese EPD basiert auf gewichteten Durchschnittswerten, die auf der Grundlage der Einzelwerte aus den verschiedenen Kingspan Insulation Fabriken ermittelt wurden. \n\nKooltherm® K3 ist ein starrer, duroplastischer, zellulärer Dämmstoff, der beidseitig mit einer glasgewebebasierten Deckschicht versehen ist. Damit der Nutzer der EPD die LCA-Ergebnisse für unterschiedliche Dicken berechnen kann, enthält die EPD die entsprechenden Berechnungsregeln. \nSystemgrenze: \nDie Art der EPD nach EN 15804 ist: Cradle to Gate mit Optionen, Modulen C1-C4 und Modul D (A1-A3, C, D und zusätzliche Module: A4, A5). \n\nDie Produktphase ist ein obligatorisches Informationsmodul und umfasst: \n- A1, Rohstoffgewinnung und -verarbeitung, Verarbeitung des sekundären Materialinputs (z.B. Recyclingprozesse), - A2, Transport zum Hersteller, - A3, Herstellung, einschließlich der Bereitstellung aller Materialien, Produkte und Energie, Verpackungsverarbeitung und deren Transport sowie Abfallverarbeitung bis zum End-of-Waste-Zustand oder Entsorgung von Endresten während der Produktphase. Die Bauprozessphase umfasst: \n- A4 Transport zur Baustelle; - A5 Einbau in das Gebäude, einschließlich der Bereitstellung aller Materialien, Produkte und Energie, sowie die Abfallverarbeitung bis zum Ende des Abfallzustands oder die Entsorgung der endgültigen Rückstände während der Bauprozessphase. Die End-of-Life-Phase ist ein obligatorisches Informationsmodul und umfasst: \n- C1 Rückbau, Abriss; - C2 Transport zur Abfallverarbeitung; - C3 Abfallverarbeitung zur Wiederverwendung, Verwertung und/oder zum Recycling; - C4 Entsorgung (nicht anwendbar für diese EPD) einschließlich Bereitstellung und aller Transporte, Bereitstellung aller Materialien, Produkte und des damit verbundenen Energie- und Wasserverbrauchs. \n\nDie Umweltbelastung durch die Verbrennung (R1 > 60 %) des Produkts am Ende des Lebenszyklus wird dem Produktsystem (C3) zugeordnet; die daraus resultierenden potenziellen Gutschriften für thermische und elektrische Energie aus der Energiesubstitution werden in Modul D angegeben. Faktoren für unterschiedliche Dicken Die in dieser EPD angegebenen LCA-Ergebnisse für das Dämmmaterial beziehen sich auf ein Produkt mit einer Dicke von 80 mm. Damit der Benutzer der EPD die Ergebnisse für verschiedene Dicken berechnen kann, können die Faktoren in der folgenden Tabelle für die Berechnung verwendet werden. Die LCA-Ergebnisse in Kapitel 5 müssen mit diesen Faktoren multipliziert werden. Die Skalierungsfaktoren gelten für das gesamte Produkt, wobei die Deckschichten für alle Produktdicken gleich sind und die Schaumstoffeinsätze mit anderen Produktdicken nach oben und unten skalieren. Hintergrunddaten aus GaBi ts Version 10 werden mit GaBi Datensätzen CUP2022.1 verwendet", "lang": "de"}], "other": {"anies": [{"name": "referenceToOriginalEPD", "value": {"shortDescription": {"value": "Kooltherm® K3 / Kooltherm® K10.pdf", "defaultValue": "Kooltherm® K3 / Kooltherm® K10.pdf", "lstrings": [{"lang": "en", "value": "Kooltherm® K3 / Kooltherm® K10.pdf"}]}, "type": "source data set", "uuid": {"uuid": "dd1be2b6-b6b9-400b-8069-b51eb44b933a"}, "refObjectId": "dd1be2b6-b6b9-400b-8069-b51eb44b933a", "resourceURLs": ["https://oekobaudat.de/OEKOBAU.DAT/resource/sources/dd1be2b6-b6b9-400b-8069-b51eb44b933a/Kooltherm_K3_Kooltherm_K10_23071.pdf?version=00.02.000"]}}]}}, "validation": {"review": [{"referenceToNameOfReviewerAndInstitution": [{"shortDescription": [{"value": "Institut Bauen und Umwelt e. V.", "lang": "en"}], "type": "contact data set", "refObjectId": "d111dbec-b024-4be5-86c5-752d6eb2cf95", "uri": "../contacts/d111dbec-b024-4be5-86c5-752d6eb2cf95.xml"}], "type": "Accredited third party review"}]}, "complianceDeclarations": {"compliance": [{"referenceToComplianceSystem": {"shortDescription": [{"value": "DIN EN 15804+A2", "lang": "en"}], "type": "source data set", "refObjectId": "c0016b33-8cf7-415c-ac6e-deba0d21440d", "uri": "../sources/c0016b33-8cf7-415c-ac6e-deba0d21440d.xml"}}, {"referenceToComplianceSystem": {"shortDescription": [{"value": "ISO 14025", "lang": "en"}], "type": "source data set", "refObjectId": "4f2eb655-6e44-4874-a95a-e28f5442cd4d", "uri": "../sources/4f2eb655-6e44-4874-a95a-e28f5442cd4d.xml"}}]}}, "administrativeInformation": {"commissionerAndGoal": {"referenceToCommissioner": [{"shortDescription": [{"value": "Kingspan Insulation B.V.", "lang": "en"}], "type": "contact data set", "refObjectId": "bdf16a2b-22c1-4001-808e-1b515e7d0d56", "uri": "../contacts/bdf16a2b-22c1-4001-808e-1b515e7d0d56.xml"}]}, "dataGenerator": {"referenceToPersonOrEntityGeneratingTheDataSet": [{"shortDescription": [{"value": "Kingspan Insulation B.V.", "lang": "en"}], "type": "contact data set", "refObjectId": "bdf16a2b-22c1-4001-808e-1b515e7d0d56", "uri": "../contacts/bdf16a2b-22c1-4001-808e-1b515e7d0d56.xml"}]}, "dataEntryBy": {"timeStamp": 1695340800000, "referenceToDataSetFormat": [{"shortDescription": [{"value": "ILCD Format", "lang": "en"}], "type": "source data set", "refObjectId": "a97a0155-0234-4b87-b4ce-a45da52f2a40", "uri": "../sources/a97a0155-0234-4b87-b4ce-a45da52f2a40.xml"}, {"shortDescription": [{"value": "EPD-Datenformaterweiterungen v1.2", "lang": "de"}, {"value": "EPD Data Format Extensions v1.2", "lang": "en"}], "type": "source data set", "refObjectId": "a29449fd-aa2f-4de8-b5d7-4b06b43c6fde", "uri": "../sources/a29449fd-aa2f-4de8-b5d7-4b06b43c6fde.xml"}]}, "publicationAndOwnership": {"dataSetVersion": "00.03.000", "referenceToPrecedingDataSetVersion": [{"shortDescription": [{"value": "Kooltherm® K3", "lang": "en"}], "type": "process data set", "refObjectId": "5aaa49cc-c5ee-4664-8a1d-6f6dbee613b1", "uri": "../processes/5aaa49cc-c5ee-4664-8a1d-6f6dbee613b1.xml"}], "referenceToRegistrationAuthority": {"shortDescription": [{"value": "Institut Bauen und Umwelt e. V.", "lang": "en"}], "type": "contact data set", "refObjectId": "d111dbec-b024-4be5-86c5-752d6eb2cf95", "uri": "../contacts/d111dbec-b024-4be5-86c5-752d6eb2cf95.xml"}, "registrationNumber": "EPD-KSI-20230322-CBA2-EN", "referenceToOwnershipOfDataSet": {"shortDescription": [{"value": "Kingspan Insulation B.V.", "lang": "en"}], "type": "contact data set", "refObjectId": "bdf16a2b-22c1-4001-808e-1b515e7d0d56", "uri": "../contacts/bdf16a2b-22c1-4001-808e-1b515e7d0d56.xml"}, "copyright": true, "licenseType": "Free of charge for all users and uses", "accessRestrictions": [{"value": "None", "lang": "en"}], "other": {"anies": [{"name": "referenceToPublisher", "value": {"shortDescription": [{"value": "Institut Bauen und Umwelt e. V.", "lang": "en"}], "type": "contact data set", "refObjectId": "d111dbec-b024-4be5-86c5-752d6eb2cf95", "uri": "../contacts/d111dbec-b024-4be5-86c5-752d6eb2cf95.xml"}}]}}}, "exchanges": {"exchange": [{"dataSetInternalID": 0, "referenceToFlowDataSet": {"shortDescription": [{"value": "Kooltherm® K3 (Kooltherm® K3)", "lang": "en"}], "type": "flow data set", "refObjectId": "e213cb4a-f1f8-474c-7f65-f1a14554da03", "uri": "../flows/e213cb4a-f1f8-474c-7f65-f1a14554da03.xml"}, "meanAmount": 1.0, "referencesToDataSource": {}, "referenceFlow": true, "resolvedFlowVersion": "00.03.000", "resultingflowAmount": 1.0, "flowProperties": [{"name": [{"lang": "de", "value": "Fläche"}, {"lang": "en", "value": "Area"}], "uuid": "93a60a56-a3c8-19da-a746-0800200c9a66", "referenceFlowProperty": true, "meanValue": 1.0, "referenceUnit": "qm", "unitGroupUUID": "c20a03d7-bd90-4569-bc94-66cfd364dfc8"}], "materialProperties": [{"name": "grammage", "value": "2.94", "unit": "kg/m^2", "unitDescription": "kilograms per square meter"}, {"name": "layer thickness", "value": "0.08", "unit": "m", "unitDescription": "meters"}], "typeOfFlow": "Product flow", "classification": {"classHierarchy": "Dämmstoffe / Phenolharz-Hartschaum (PF) / PF-Platten", "name": "OEKOBAU.DAT"}}, {"dataSetInternalID": 1, "referenceToFlowDataSet": {"shortDescription": [{"value": "Renewable primary energy as energy carrier (PERE)", "lang": "en"}, {"value": "Erneuerbare Primärenergie als Energieträger (PERE)", "lang": "de"}], "type": "flow data set", "refObjectId": "20f32be5-0398-4288-9b6d-accddd195317", "uri": "../flows/20f32be5-0398-4288-9b6d-accddd195317.xml"}, "exchange direction": "INPUT", "other": {"anies": [{"name": "referenceToUnitGroupDataSet", "value": {"shortDescription": [{"value": "MJ", "lang": "en"}], "type": "unit group data set", "refObjectId": "93a60a57-a3c8-11da-a746-0800200c9a66", "uri": "../unitgroups/93a60a57-a3c8-11da-a746-0800200c9a66.xml"}}, {"value": "20.5829401998409", "module": "A1-A3"}, {"value": "0.0187293983424805", "module": "A4"}, {"value": "0.0141809051701026", "module": "A5"}, {"value": "9.62602611768205E-05", "module": "C1"}, {"value": "0.00936469917124023", "module": "C2"}, {"value": "0.288715466237046", "module": "C3"}, {"value": "0", "module": "C4"}, {"value": "-11.8203449047548", "module": "D"}]}, "resolvedFlowVersion": "38.00.000", "flowProperties": [], "typeOfFlow": "Other flow", "classification": {"classHierarchy": "Quantities", "name": "GaBiCategories"}}, {"dataSetInternalID": 2, "referenceToFlowDataSet": {"shortDescription": [{"value": "Renewable primary energy resources as material utilization (PERM)", "lang": "en"}, {"value": "Erneuerbare Primärenergie zur stofflichen Nutzung (PERM)", "lang": "de"}], "type": "flow data set", "refObjectId": "fb3ec0de-548d-4508-aea5-00b73bf6f702", "uri": "../flows/fb3ec0de-548d-4508-aea5-00b73bf6f702.xml"}, "exchange direction": "INPUT", "other": {"anies": [{"name": "referenceToUnitGroupDataSet", "value": {"shortDescription": [{"value": "MJ", "lang": "en"}], "type": "unit group data set", "refObjectId": "93a60a57-a3c8-11da-a746-0800200c9a66", "uri": "../unitgroups/93a60a57-a3c8-11da-a746-0800200c9a66.xml"}}, {"value": "0", "module": "A1-A3"}, {"value": "0", "module": "A4"}, {"value": "0", "module": "A5"}, {"value": "0", "module": "C1"}, {"value": "0", "module": "C2"}, {"value": "0", "module": "C3"}, {"value": "0", "module": "C4"}, {"value": "0", "module": "D"}]}, "resolvedFlowVersion": "38.00.000", "flowProperties": [], "typeOfFlow": "Other flow", "classification": {"classHierarchy": "Quantities", "name": "GaBiCategories"}}, {"dataSetInternalID": 3, "referenceToFlowDataSet": {"shortDescription": [{"value": "Total use of renewable primary energy resources (PERT)", "lang": "en"}, {"value": "Total erneuerbare Primärenergie (PERT)", "lang": "de"}], "type": "flow data set", "refObjectId": "53f97275-fa8a-4cdd-9024-65936002acd0", "uri": "../flows/53f97275-fa8a-4cdd-9024-65936002acd0.xml"}, "exchange direction": "INPUT", "other": {"anies": [{"name": "referenceToUnitGroupDataSet", "value": {"shortDescription": [{"value": "MJ", "lang": "en"}], "type": "unit group data set", "refObjectId": "93a60a57-a3c8-11da-a746-0800200c9a66", "uri": "../unitgroups/93a60a57-a3c8-11da-a746-0800200c9a66.xml"}}, {"value": "20.5829401998409", "module": "A1-A3"}, {"value": "0.0187293983424805", "module": "A4"}, {"value": "0.0141809051701026", "module": "A5"}, {"value": "9.62602611768205E-05", "module": "C1"}, {"value": "0.00936469917124023", "module": "C2"}, {"value": "0.288715466237046", "module": "C3"}, {"value": "0", "module": "C4"}, {"value": "-11.8203449047548", "module": "D"}]}, "resolvedFlowVersion": "38.00.000", "flowProperties": [], "typeOfFlow": "Other flow", "classification": {"classHierarchy": "Quantities / Environmental quantities / EPD EN 15804 / LCI indicators", "name": "GaBiCategories"}}, {"dataSetInternalID": 4, "referenceToFlowDataSet": {"shortDescription": [{"value": "Non renewable primary energy as energy carrier (PENRE)", "lang": "en"}, {"value": "Nicht-erneuerbare Primärenergie als Energieträger (PENRE)", "lang": "de"}], "type": "flow data set", "refObjectId": "ac857178-2b45-46ec-892a-a9a4332f0372", "uri": "../flows/ac857178-2b45-46ec-892a-a9a4332f0372.xml"}, "exchange direction": "INPUT", "other": {"anies": [{"name": "referenceToUnitGroupDataSet", "value": {"shortDescription": [{"value": "MJ", "lang": "en"}], "type": "unit group data set", "refObjectId": "93a60a57-a3c8-11da-a746-0800200c9a66", "uri": "../unitgroups/93a60a57-a3c8-11da-a746-0800200c9a66.xml"}}, {"value": "78.7913645113369", "module": "A1-A3"}, {"value": "0.330247982926438", "module": "A4"}, {"value": "2.60485421813606", "module": "A5"}, {"value": "0.0255452597307703", "module": "C1"}, {"value": "0.16512399146322", "module": "C2"}, {"value": "81.8516027656965", "module": "C3"}, {"value": "0", "module": "C4"}, {"value": "-42.9363043360743", "module": "D"}]}, "resolvedFlowVersion": "38.00.000", "flowProperties": [], "typeOfFlow": "Other flow", "classification": {"classHierarchy": "Quantities", "name": "GaBiCategories"}}, {"dataSetInternalID": 5, "referenceToFlowDataSet": {"shortDescription": [{"value": "Non renewable primary energy as material utilization (PENRM)", "lang": "en"}, {"value": "Nicht-erneuerbare Primärenergie zur stofflichen Nutzung (PENRM)", "lang": "de"}], "type": "flow data set", "refObjectId": "1421caa0-679d-4bf4-b282-0eb850ccae27", "uri": "../flows/1421caa0-679d-4bf4-b282-0eb850ccae27.xml"}, "exchange direction": "INPUT", "other": {"anies": [{"name": "referenceToUnitGroupDataSet", "value": {"shortDescription": [{"value": "MJ", "lang": "en"}], "type": "unit group data set", "refObjectId": "93a60a57-a3c8-11da-a746-0800200c9a66", "uri": "../unitgroups/93a60a57-a3c8-11da-a746-0800200c9a66.xml"}}, {"value": "82.74302", "module": "A1-A3"}, {"value": "0", "module": "A4"}, {"value": "-2.5496", "module": "A5"}, {"value": "0", "module": "C1"}, {"value": "0", "module": "C2"}, {"value": "-80.19342", "module": "C3"}, {"value": "0", "module": "C4"}, {"value": "0", "module": "D"}]}, "resolvedFlowVersion": "38.00.000", "flowProperties": [], "typeOfFlow": "Other flow", "classification": {"classHierarchy": "Quantities", "name": "GaBiCategories"}}, {"dataSetInternalID": 6, "referenceToFlowDataSet": {"shortDescription": [{"value": "Total use of non renewable primary energy resources (PENRT)", "lang": "en"}, {"value": "Total nicht erneuerbare Primärenergie (PENRT)", "lang": "de"}], "type": "flow data set", "refObjectId": "06159210-646b-4c8d-8583-da9b3b95a6c1", "uri": "../flows/06159210-646b-4c8d-8583-da9b3b95a6c1.xml"}, "exchange direction": "INPUT", "other": {"anies": [{"name": "referenceToUnitGroupDataSet", "value": {"shortDescription": [{"value": "MJ", "lang": "en"}], "type": "unit group data set", "refObjectId": "93a60a57-a3c8-11da-a746-0800200c9a66", "uri": "../unitgroups/93a60a57-a3c8-11da-a746-0800200c9a66.xml"}}, {"value": "161.534384511338", "module": "A1-A3"}, {"value": "0.330247982926438", "module": "A4"}, {"value": "0.0552542181360639", "module": "A5"}, {"value": "0.0255452597307704", "module": "C1"}, {"value": "0.16512399146322", "module": "C2"}, {"value": "1.65818276569655", "module": "C3"}, {"value": "0", "module": "C4"}, {"value": "-42.9363043360746", "module": "D"}]}, "resolvedFlowVersion": "38.00.000", "flowProperties": [], "typeOfFlow": "Other flow", "classification": {"classHierarchy": "Quantities / Environmental quantities / EPD EN 15804 / LCI indicators", "name": "GaBiCategories"}}, {"dataSetInternalID": 7, "referenceToFlowDataSet": {"shortDescription": [{"value": "Use of secondary material (SM)", "lang": "en"}, {"value": "Einsatz von Sekundärstoffen (SM)", "lang": "de"}], "type": "flow data set", "refObjectId": "c6a1f35f-2d09-4f54-8dfb-97e502e1ce92", "uri": "../flows/c6a1f35f-2d09-4f54-8dfb-97e502e1ce92.xml"}, "exchange direction": "INPUT", "other": {"anies": [{"name": "referenceToUnitGroupDataSet", "value": {"shortDescription": [{"value": "kg", "lang": "en"}], "type": "unit group data set", "refObjectId": "ad38d542-3fe9-439d-9b95-2f5f7752acaf", "uri": "../unitgroups/ad38d542-3fe9-439d-9b95-2f5f7752acaf.xml"}}, {"value": "0", "module": "A1-A3"}, {"value": "0", "module": "A4"}, {"value": "0", "module": "A5"}, {"value": "0", "module": "C1"}, {"value": "0", "module": "C2"}, {"value": "0", "module": "C3"}, {"value": "0", "module": "C4"}, {"value": "0", "module": "D"}]}, "resolvedFlowVersion": "38.00.000", "flowProperties": [], "typeOfFlow": "Other flow", "classification": {"classHierarchy": "Quantities / Environmental quantities / EPD EN 15804 / LCI indicators", "name": "GaBiCategories"}}, {"dataSetInternalID": 8, "referenceToFlowDataSet": {"shortDescription": [{"value": "Use of renewable secondary fuels (RSF)", "lang": "en"}, {"value": "Erneuerbare Sekundärbrennstoffe (RSF)", "lang": "de"}], "type": "flow data set", "refObjectId": "64333088-a55f-4aa2-9a31-c10b07816787", "uri": "../flows/64333088-a55f-4aa2-9a31-c10b07816787.xml"}, "exchange direction": "INPUT", "other": {"anies": [{"name": "referenceToUnitGroupDataSet", "value": {"shortDescription": [{"value": "MJ", "lang": "en"}], "type": "unit group data set", "refObjectId": "93a60a57-a3c8-11da-a746-0800200c9a66", "uri": "../unitgroups/93a60a57-a3c8-11da-a746-0800200c9a66.xml"}}, {"value": "0", "module": "A1-A3"}, {"value": "0", "module": "A4"}, {"value": "0", "module": "A5"}, {"value": "0", "module": "C1"}, {"value": "0", "module": "C2"}, {"value": "0", "module": "C3"}, {"value": "0", "module": "C4"}, {"value": "0", "module": "D"}]}, "resolvedFlowVersion": "38.00.000", "flowProperties": [], "typeOfFlow": "Other flow", "classification": {"classHierarchy": "Quantities / Environmental quantities / EPD EN 15804 / LCI indicators", "name": "GaBiCategories"}}, {"dataSetInternalID": 9, "referenceToFlowDataSet": {"shortDescription": [{"value": "Use of non renewable secondary fuels (NRSF)", "lang": "en"}, {"value": "Nicht erneuerbare Sekundärbrennstoffe (NRSF)", "lang": "de"}], "type": "flow data set", "refObjectId": "89def144-d39a-4287-b86f-efde453ddcb2", "uri": "../flows/89def144-d39a-4287-b86f-efde453ddcb2.xml"}, "exchange direction": "INPUT", "other": {"anies": [{"name": "referenceToUnitGroupDataSet", "value": {"shortDescription": [{"value": "MJ", "lang": "en"}], "type": "unit group data set", "refObjectId": "93a60a57-a3c8-11da-a746-0800200c9a66", "uri": "../unitgroups/93a60a57-a3c8-11da-a746-0800200c9a66.xml"}}, {"value": "0", "module": "A1-A3"}, {"value": "0", "module": "A4"}, {"value": "0", "module": "A5"}, {"value": "0", "module": "C1"}, {"value": "0", "module": "C2"}, {"value": "0", "module": "C3"}, {"value": "0", "module": "C4"}, {"value": "0", "module": "D"}]}, "resolvedFlowVersion": "38.00.000", "flowProperties": [], "typeOfFlow": "Other flow", "classification": {"classHierarchy": "Quantities / Environmental quantities / EPD EN 15804 / LCI indicators", "name": "GaBiCategories"}}, {"dataSetInternalID": 10, "referenceToFlowDataSet": {"shortDescription": [{"value": "Use of net fresh water (FW)", "lang": "en"}, {"value": "Einsatz von Süßwasserressourcen (FW)", "lang": "de"}], "type": "flow data set", "refObjectId": "3cf952c8-f3a4-461d-8c96-96456ca62246", "uri": "../flows/3cf952c8-f3a4-461d-8c96-96456ca62246.xml"}, "exchange direction": "INPUT", "other": {"anies": [{"name": "referenceToUnitGroupDataSet", "value": {"shortDescription": [{"value": "m^3", "lang": "en"}], "type": "unit group data set", "refObjectId": "cd950537-0a98-4044-9ba7-9f9a68d0a504", "uri": "../unitgroups/cd950537-0a98-4044-9ba7-9f9a68d0a504.xml"}}, {"value": "0.0350286530732981", "module": "A1-A3"}, {"value": "2.11819953655159E-05", "module": "A4"}, {"value": "0.000336970140431998", "module": "A5"}, {"value": "1.4518394000734E-07", "module": "C1"}, {"value": "1.05909976827579E-05", "module": "C2"}, {"value": "0.0148867275725975", "module": "C3"}, {"value": "0", "module": "C4"}, {"value": "-0.0113626888162261", "module": "D"}]}, "resolvedFlowVersion": "38.00.000", "flowProperties": [], "typeOfFlow": "Other flow", "classification": {"classHierarchy": "Quantities / Environmental quantities / EPD EN 15804 / LCI indicators", "name": "GaBiCategories"}}, {"dataSetInternalID": 11, "referenceToFlowDataSet": {"shortDescription": [{"value": "Hazardous waste disposed (HWD)", "lang": "en"}, {"value": "Gefährlicher Abfall zur Deponie (HWD)", "lang": "de"}], "type": "flow data set", "refObjectId": "430f9e0f-59b2-46a0-8e0d-55e0e84948fc", "uri": "../flows/430f9e0f-59b2-46a0-8e0d-55e0e84948fc.xml"}, "exchange direction": "OUTPUT", "other": {"anies": [{"name": "referenceToUnitGroupDataSet", "value": {"shortDescription": [{"value": "kg", "lang": "en"}], "type": "unit group data set", "refObjectId": "ad38d542-3fe9-439d-9b95-2f5f7752acaf", "uri": "../unitgroups/ad38d542-3fe9-439d-9b95-2f5f7752acaf.xml"}}, {"value": "7.65271012904991E-05", "module": "A1-A3"}, {"value": "1.58147820933287E-12", "module": "A4"}, {"value": "4.60237872693301E-12", "module": "A5"}, {"value": "8.4353223694102E-14", "module": "C1"}, {"value": "7.90739104666434E-13", "module": "C2"}, {"value": "2.28513954232676E-10", "module": "C3"}, {"value": "0", "module": "C4"}, {"value": "-5.80778420892083E-09", "module": "D"}]}, "resolvedFlowVersion": "38.00.000", "flowProperties": [], "typeOfFlow": "Other flow", "classification": {"classHierarchy": "Quantities / Environmental quantities / EPD EN 15804 / LCI indicators", "name": "GaBiCategories"}}, {"dataSetInternalID": 12, "referenceToFlowDataSet": {"shortDescription": [{"value": "Non hazardous waste disposed (NHWD)", "lang": "en"}, {"value": "Entsorgter nicht gefährlicher Abfall (NHWD)", "lang": "de"}], "type": "flow data set", "refObjectId": "b29ef66b-e286-4afa-949f-62f1a7b4d7fa", "uri": "../flows/b29ef66b-e286-4afa-949f-62f1a7b4d7fa.xml"}, "exchange direction": "OUTPUT", "other": {"anies": [{"name": "referenceToUnitGroupDataSet", "value": {"shortDescription": [{"value": "kg", "lang": "en"}], "type": "unit group data set", "refObjectId": "ad38d542-3fe9-439d-9b95-2f5f7752acaf", "uri": "../unitgroups/ad38d542-3fe9-439d-9b95-2f5f7752acaf.xml"}}, {"value": "0.0866550859924144", "module": "A1-A3"}, {"value": "4.73293016940511E-05", "module": "A4"}, {"value": "0.0134462725532853", "module": "A5"}, {"value": "2.39151217688407E-06", "module": "C1"}, {"value": "2.36646508470255E-05", "module": "C2"}, {"value": "0.032336513883232", "module": "C3"}, {"value": "0", "module": "C4"}, {"value": "-0.0217181940746453", "module": "D"}]}, "resolvedFlowVersion": "38.00.000", "flowProperties": [], "typeOfFlow": "Other flow", "classification": {"classHierarchy": "Quantities / Environmental quantities / EPD EN 15804 / LCI indicators", "name": "GaBiCategories"}}, {"dataSetInternalID": 13, "referenceToFlowDataSet": {"shortDescription": [{"value": "Radioactive waste disposed (RWD)", "lang": "en"}, {"value": "Entsorgter radioaktiver Abfall (RWD)", "lang": "de"}], "type": "flow data set", "refObjectId": "3449546e-52ad-4b39-b809-9fb77cea8ff6", "uri": "../flows/3449546e-52ad-4b39-b809-9fb77cea8ff6.xml"}, "exchange direction": "OUTPUT", "other": {"anies": [{"name": "referenceToUnitGroupDataSet", "value": {"shortDescription": [{"value": "kg", "lang": "en"}], "type": "unit group data set", "refObjectId": "ad38d542-3fe9-439d-9b95-2f5f7752acaf", "uri": "../unitgroups/ad38d542-3fe9-439d-9b95-2f5f7752acaf.xml"}}, {"value": "0.00184326654389594", "module": "A1-A3"}, {"value": "4.06758110751738E-07", "module": "A4"}, {"value": "2.29902682157053E-06", "module": "A5"}, {"value": "2.79950385672721E-08", "module": "C1"}, {"value": "2.03379055375869E-07", "module": "C2"}, {"value": "6.84641269115478E-05", "module": "C3"}, {"value": "0", "module": "C4"}, {"value": "-0.00338960201423844", "module": "D"}]}, "resolvedFlowVersion": "38.00.000", "flowProperties": [], "typeOfFlow": "Other flow", "classification": {"classHierarchy": "Quantities / Environmental quantities / EPD EN 15804 / LCI indicators", "name": "GaBiCategories"}}, {"dataSetInternalID": 14, "referenceToFlowDataSet": {"shortDescription": [{"value": "Components for re-use (CRU)", "lang": "en"}, {"value": "Komponenten für die Wiederverwendung (CRU)", "lang": "de"}], "type": "flow data set", "refObjectId": "a2b32f97-3fc7-4af2-b209-525bc6426f33", "uri": "../flows/a2b32f97-3fc7-4af2-b209-525bc6426f33.xml"}, "exchange direction": "OUTPUT", "other": {"anies": [{"name": "referenceToUnitGroupDataSet", "value": {"shortDescription": [{"value": "kg", "lang": "en"}], "type": "unit group data set", "refObjectId": "ad38d542-3fe9-439d-9b95-2f5f7752acaf", "uri": "../unitgroups/ad38d542-3fe9-439d-9b95-2f5f7752acaf.xml"}}, {"value": "0", "module": "A1-A3"}, {"value": "0", "module": "A4"}, {"value": "0", "module": "A5"}, {"value": "0", "module": "C1"}, {"value": "0", "module": "C2"}, {"value": "0", "module": "C3"}, {"value": "0", "module": "C4"}, {"value": "0", "module": "D"}]}, "resolvedFlowVersion": "38.00.000", "flowProperties": [], "typeOfFlow": "Other flow", "classification": {"classHierarchy": "Quantities / Environmental quantities / EPD EN 15804 / LCI indicators", "name": "GaBiCategories"}}, {"dataSetInternalID": 15, "referenceToFlowDataSet": {"shortDescription": [{"value": "Materials for recycling (MFR)", "lang": "en"}, {"value": "Stoffe zum Recycling (MFR)", "lang": "de"}], "type": "flow data set", "refObjectId": "d7fe48a5-4103-49c8-9aae-b0b5dfdbd6ae", "uri": "../flows/d7fe48a5-4103-49c8-9aae-b0b5dfdbd6ae.xml"}, "exchange direction": "OUTPUT", "other": {"anies": [{"name": "referenceToUnitGroupDataSet", "value": {"shortDescription": [{"value": "kg", "lang": "en"}], "type": "unit group data set", "refObjectId": "ad38d542-3fe9-439d-9b95-2f5f7752acaf", "uri": "../unitgroups/ad38d542-3fe9-439d-9b95-2f5f7752acaf.xml"}}, {"value": "0", "module": "A1-A3"}, {"value": "0", "module": "A4"}, {"value": "0", "module": "A5"}, {"value": "0", "module": "C1"}, {"value": "0", "module": "C2"}, {"value": "0", "module": "C3"}, {"value": "0", "module": "C4"}, {"value": "0", "module": "D"}]}, "resolvedFlowVersion": "38.00.000", "flowProperties": [], "typeOfFlow": "Other flow", "classification": {"classHierarchy": "Quantities / Environmental quantities / EPD EN 15804 / LCI indicators", "name": "GaBiCategories"}}, {"dataSetInternalID": 16, "referenceToFlowDataSet": {"shortDescription": [{"value": "Materials for energy recovery (MER)", "lang": "en"}, {"value": "Stoffe für die Energierückgewinnung (MER)", "lang": "de"}], "type": "flow data set", "refObjectId": "59a9181c-3aaf-46ee-8b13-2b3723b6e447", "uri": "../flows/59a9181c-3aaf-46ee-8b13-2b3723b6e447.xml"}, "exchange direction": "OUTPUT", "other": {"anies": [{"name": "referenceToUnitGroupDataSet", "value": {"shortDescription": [{"value": "kg", "lang": "en"}], "type": "unit group data set", "refObjectId": "ad38d542-3fe9-439d-9b95-2f5f7752acaf", "uri": "../unitgroups/ad38d542-3fe9-439d-9b95-2f5f7752acaf.xml"}}, {"value": "0", "module": "A1-A3"}, {"value": "0", "module": "A4"}, {"value": "0.0599", "module": "A5"}, {"value": "0", "module": "C1"}, {"value": "0", "module": "C2"}, {"value": "2.912", "module": "C3"}, {"value": "0", "module": "C4"}, {"value": "0", "module": "D"}]}, "resolvedFlowVersion": "38.00.000", "flowProperties": [], "typeOfFlow": "Other flow", "classification": {"classHierarchy": "Quantities / Environmental quantities / EPD EN 15804 / LCI indicators", "name": "GaBiCategories"}}, {"dataSetInternalID": 17, "referenceToFlowDataSet": {"shortDescription": [{"value": "Exported electrical energy (EEE)", "lang": "en"}, {"value": "Exportierte elektrische Energie (EEE)", "lang": "de"}], "type": "flow data set", "refObjectId": "4da0c987-2b76-40d6-9e9e-82a017aaaf29", "uri": "../flows/4da0c987-2b76-40d6-9e9e-82a017aaaf29.xml"}, "exchange direction": "OUTPUT", "other": {"anies": [{"name": "referenceToUnitGroupDataSet", "value": {"shortDescription": [{"value": "MJ", "lang": "en"}], "type": "unit group data set", "refObjectId": "93a60a57-a3c8-11da-a746-0800200c9a66", "uri": "../unitgroups/93a60a57-a3c8-11da-a746-0800200c9a66.xml"}}, {"value": "0", "module": "A1-A3"}, {"value": "0", "module": "A4"}, {"value": "0.271654862038036", "module": "A5"}, {"value": "0", "module": "C1"}, {"value": "0", "module": "C2"}, {"value": "11.1090002636484", "module": "C3"}, {"value": "0", "module": "C4"}, {"value": "0", "module": "D"}]}, "resolvedFlowVersion": "38.00.000", "flowProperties": [], "typeOfFlow": "Other flow", "classification": {"classHierarchy": "Quantities / Environmental quantities / EPD EN 15804 / LCI indicators", "name": "GaBiCategories"}}, {"dataSetInternalID": 18, "referenceToFlowDataSet": {"shortDescription": [{"value": "Exported thermal energy (EET)", "lang": "en"}, {"value": "Exportierte thermische Energie (EET)", "lang": "de"}], "type": "flow data set", "refObjectId": "98daf38a-7a79-46d3-9a37-2b7bd0955810", "uri": "../flows/98daf38a-7a79-46d3-9a37-2b7bd0955810.xml"}, "exchange direction": "OUTPUT", "other": {"anies": [{"name": "referenceToUnitGroupDataSet", "value": {"shortDescription": [{"value": "MJ", "lang": "en"}], "type": "unit group data set", "refObjectId": "93a60a57-a3c8-11da-a746-0800200c9a66", "uri": "../unitgroups/93a60a57-a3c8-11da-a746-0800200c9a66.xml"}}, {"value": "0", "module": "A1-A3"}, {"value": "0", "module": "A4"}, {"value": "0.486071022629257", "module": "A5"}, {"value": "0", "module": "C1"}, {"value": "0", "module": "C2"}, {"value": "19.8717449528625", "module": "C3"}, {"value": "0", "module": "C4"}, {"value": "0", "module": "D"}]}, "resolvedFlowVersion": "38.00.000", "flowProperties": [], "typeOfFlow": "Other flow", "classification": {"classHierarchy": "Quantities / Environmental quantities / EPD EN 15804 / LCI indicators", "name": "GaBiCategories"}}]}, "LCIAResults": {"LCIAResult": [{"referenceToLCIAMethodDataSet": {"shortDescription": [{"value": "Global Warming Potential total (GWP-total)", "lang": "en"}, {"value": "Globales Erwärmungspotenzial total (GWP-total)", "lang": "de"}], "type": "LCIA method data set", "refObjectId": "6a37f984-a4b3-458a-a20a-64418c145fa2", "uri": "../lciamethods/6a37f984-a4b3-458a-a20a-64418c145fa2.xml"}, "other": {"anies": [{"name": "referenceToUnitGroupDataSet", "value": {"shortDescription": [{"value": "kg CO_(2) eq", "lang": "en"}], "type": "unit group data set", "refObjectId": "1ebf3012-d0db-4de2-aefd-ef30cedb0be1", "uri": "../unitgroups/1ebf3012-d0db-4de2-aefd-ef30cedb0be1.xml"}}, {"value": "5.56231381746199", "module": "A1-A3"}, {"value": "0.0247486456984539", "module": "A4"}, {"value": "0.149639581902304", "module": "A5"}, {"value": "0.00188635071425881", "module": "C1"}, {"value": "0.0123743228492269", "module": "C2"}, {"value": "6.42568994867864", "module": "C3"}, {"value": "0", "module": "C4"}, {"value": "-2.53699437588649", "module": "D"}]}}, {"referenceToLCIAMethodDataSet": {"shortDescription": [{"value": "Global Warming Potential fossil fuels (GWP-fossil)", "lang": "en"}, {"value": "Globales Erwärmungspotenzial fossil (GWP-fossil)", "lang": "de"}], "type": "LCIA method data set", "refObjectId": "5f635281-343e-44fb-83df-1971b155e6b6", "uri": "../lciamethods/5f635281-343e-44fb-83df-1971b155e6b6.xml"}, "other": {"anies": [{"name": "referenceToUnitGroupDataSet", "value": {"shortDescription": [{"value": "kg CO_(2) eq", "lang": "en"}], "type": "unit group data set", "refObjectId": "1ebf3012-d0db-4de2-aefd-ef30cedb0be1", "uri": "../unitgroups/1ebf3012-d0db-4de2-aefd-ef30cedb0be1.xml"}}, {"value": "5.53683931861581", "module": "A1-A3"}, {"value": "0.024645247793672", "module": "A4"}, {"value": "0.149629634357101", "module": "A5"}, {"value": "0.00188380623609957", "module": "C1"}, {"value": "0.012322623896836", "module": "C2"}, {"value": "6.42524162813633", "module": "C3"}, {"value": "0", "module": "C4"}, {"value": "-2.52378333681911", "module": "D"}]}}, {"referenceToLCIAMethodDataSet": {"shortDescription": [{"value": "Global Warming Potential biogenic (GWP-biogenic)", "lang": "en"}, {"value": "Globales Erwärmungspotenzial biogen (GWP-biogenic)", "lang": "de"}], "type": "LCIA method data set", "refObjectId": "2356e1ab-0185-4db5-86e5-16de51c7485c", "uri": "../lciamethods/2356e1ab-0185-4db5-86e5-16de51c7485c.xml"}, "other": {"anies": [{"name": "referenceToUnitGroupDataSet", "value": {"shortDescription": [{"value": "kg CO_(2) eq", "lang": "en"}], "type": "unit group data set", "refObjectId": "1ebf3012-d0db-4de2-aefd-ef30cedb0be1", "uri": "../unitgroups/1ebf3012-d0db-4de2-aefd-ef30cedb0be1.xml"}}, {"value": "-0.038369790965263", "module": "A1-A3"}, {"value": "-3.40518069572119E-05", "module": "A4"}, {"value": "8.17292109437323E-06", "module": "A5"}, {"value": "2.52123251223559E-06", "module": "C1"}, {"value": "-1.7025903478606E-05", "module": "C2"}, {"value": "0.000436909073700055", "module": "C3"}, {"value": "0", "module": "C4"}, {"value": "-0.0129330259067353", "module": "D"}]}}, {"referenceToLCIAMethodDataSet": {"shortDescription": [{"value": "Global Warming Potential luluc (GWP-luluc)", "lang": "en"}, {"value": "Globales Erwärmungspotenzial luluc (GWP-luluc)", "lang": "de"}], "type": "LCIA method data set", "refObjectId": "4331bbdb-978a-490d-8707-eeb047f01a55", "uri": "../lciamethods/4331bbdb-978a-490d-8707-eeb047f01a55.xml"}, "other": {"anies": [{"name": "referenceToUnitGroupDataSet", "value": {"shortDescription": [{"value": "kg CO_(2) eq", "lang": "en"}], "type": "unit group data set", "refObjectId": "1ebf3012-d0db-4de2-aefd-ef30cedb0be1", "uri": "../unitgroups/1ebf3012-d0db-4de2-aefd-ef30cedb0be1.xml"}}, {"value": "0.0638442898114389", "module": "A1-A3"}, {"value": "0.000137449711739037", "module": "A4"}, {"value": "1.77462410925597E-06", "module": "A5"}, {"value": "2.32456470100896E-08", "module": "C1"}, {"value": "6.87248558695187E-05", "module": "C2"}, {"value": "1.14114686075805E-05", "module": "C3"}, {"value": "0", "module": "C4"}, {"value": "-0.000278013160638414", "module": "D"}]}}, {"referenceToLCIAMethodDataSet": {"shortDescription": [{"value": "Depletion potential of the stratospheric ozone layer (ODP)", "lang": "en"}, {"value": "Abbau Potential der stratosphärischen Ozonschicht (ODP)", "lang": "de"}], "type": "LCIA method data set", "refObjectId": "b5c629d6-def3-11e6-bf01-fe55135034f3", "uri": "../lciamethods/b5c629d6-def3-11e6-bf01-fe55135034f3.xml"}, "other": {"anies": [{"name": "referenceToUnitGroupDataSet", "value": {"shortDescription": [{"value": "kg CFC11 eq", "lang": "en"}], "type": "unit group data set", "refObjectId": "d9e957c9-7309-4474-bf3a-7777df6c4e5b", "uri": "../unitgroups/d9e957c9-7309-4474-bf3a-7777df6c4e5b.xml"}}, {"value": "1.13858106251525E-08", "module": "A1-A3"}, {"value": "1.47704329125363E-15", "module": "A4"}, {"value": "2.66235555491071E-14", "module": "A5"}, {"value": "1.15554320079412E-16", "module": "C1"}, {"value": "7.38521645626814E-16", "module": "C2"}, {"value": "4.70493679868544E-13", "module": "C3"}, {"value": "0", "module": "C4"}, {"value": "-1.71106069922974E-11", "module": "D"}]}}, {"referenceToLCIAMethodDataSet": {"shortDescription": [{"value": "Acidification potential of land and water (AP)", "lang": "en"}, {"value": "Versauerungspotenzial von Boden und Wasser (AP)", "lang": "de"}], "type": "LCIA method data set", "refObjectId": "b5c611c6-def3-11e6-bf01-fe55135034f3", "uri": "../lciamethods/b5c611c6-def3-11e6-bf01-fe55135034f3.xml"}, "other": {"anies": [{"name": "referenceToUnitGroupDataSet", "value": {"shortDescription": [{"value": "mol H^(+) eq", "lang": "en"}], "type": "unit group data set", "refObjectId": "42e089ac-92bf-4bf2-8ca1-5fc40d18f2ed", "uri": "../unitgroups/42e089ac-92bf-4bf2-8ca1-5fc40d18f2ed.xml"}}, {"value": "0.0112926090150747", "module": "A1-A3"}, {"value": "2.5401915165722E-05", "module": "A4"}, {"value": "1.86440176228313E-05", "module": "A5"}, {"value": "8.75110299470448E-06", "module": "C1"}, {"value": "1.27009575828611E-05", "module": "C2"}, {"value": "0.00379127765421747", "module": "C3"}, {"value": "0", "module": "C4"}, {"value": "-0.00332503071888471", "module": "D"}]}}, {"referenceToLCIAMethodDataSet": {"shortDescription": [{"value": "Eutrophication potential aquatic freshwater (EP-freshwater)", "lang": "en"}, {"value": "Eutrophierungspotenzial Süßwasser (EP-freshwater)", "lang": "de"}], "type": "LCIA method data set", "refObjectId": "b53ec18f-7377-4ad3-86eb-cc3f4f276b2b", "uri": "../lciamethods/b53ec18f-7377-4ad3-86eb-cc3f4f276b2b.xml"}, "other": {"anies": [{"name": "referenceToUnitGroupDataSet", "value": {"shortDescription": [{"value": "kg P eq", "lang": "en"}], "type": "unit group data set", "refObjectId": "0429039d-a61d-4590-ba67-aa4a20a810a1", "uri": "../unitgroups/0429039d-a61d-4590-ba67-aa4a20a810a1.xml"}}, {"value": "1.86981070785541E-05", "module": "A1-A3"}, {"value": "7.35898018086318E-08", "module": "A4"}, {"value": "6.725819876753E-09", "module": "A5"}, {"value": "3.80011067033517E-10", "module": "C1"}, {"value": "3.67949009043159E-08", "module": "C2"}, {"value": "1.26681536570973E-07", "module": "C3"}, {"value": "0", "module": "C4"}, {"value": "-3.48120833452775E-06", "module": "D"}]}}, {"referenceToLCIAMethodDataSet": {"shortDescription": [{"value": "Eutrophication potential aquatic marine (EP-marine)", "lang": "en"}, {"value": "Eutrophierungspotenzial Salzwasser (EP-marine)", "lang": "de"}], "type": "LCIA method data set", "refObjectId": "b5c619fa-def3-11e6-bf01-fe55135034f3", "uri": "../lciamethods/b5c619fa-def3-11e6-bf01-fe55135034f3.xml"}, "other": {"anies": [{"name": "referenceToUnitGroupDataSet", "value": {"shortDescription": [{"value": "kg N eq", "lang": "en"}], "type": "unit group data set", "refObjectId": "d05bb823-ecdf-4686-8c40-bf1d9257859f", "uri": "../unitgroups/d05bb823-ecdf-4686-8c40-bf1d9257859f.xml"}}, {"value": "0.00318139923131015", "module": "A1-A3"}, {"value": "8.31048989482905E-06", "module": "A4"}, {"value": "4.99872995442769E-06", "module": "A5"}, {"value": "4.16788765172823E-06", "module": "C1"}, {"value": "4.15524494741453E-06", "module": "C2"}, {"value": "0.0018355875310265", "module": "C3"}, {"value": "0", "module": "C4"}, {"value": "-0.000901465603647013", "module": "D"}]}}, {"referenceToLCIAMethodDataSet": {"shortDescription": [{"value": "Eutrophication potential terrestrial (EP-terrestrial)", "lang": "en"}, {"value": "Eutrophierungspotenzial Land (EP-terrestrial)", "lang": "de"}], "type": "LCIA method data set", "refObjectId": "b5c614d2-def3-11e6-bf01-fe55135034f3", "uri": "../lciamethods/b5c614d2-def3-11e6-bf01-fe55135034f3.xml"}, "other": {"anies": [{"name": "referenceToUnitGroupDataSet", "value": {"shortDescription": [{"value": "mol N eq", "lang": "en"}], "type": "unit group data set", "refObjectId": "71b4d617-0ec9-4d3f-b65e-e438940c2401", "uri": "../unitgroups/71b4d617-0ec9-4d3f-b65e-e438940c2401.xml"}}, {"value": "0.0316145222684203", "module": "A1-A3"}, {"value": "9.8923970345706E-05", "module": "A4"}, {"value": "8.47814729926004E-05", "module": "A5"}, {"value": "4.56506665276497E-05", "module": "C1"}, {"value": "4.9461985172853E-05", "module": "C2"}, {"value": "0.0211227645546819", "module": "C3"}, {"value": "0", "module": "C4"}, {"value": "-0.00965406991793713", "module": "D"}]}}, {"referenceToLCIAMethodDataSet": {"shortDescription": [{"value": "Formation potential of tropospheric ozone photochemical oxidants (POCP)", "lang": "en"}, {"value": "Bildungspotential für troposphärisches Ozon (POCP)", "lang": "de"}], "type": "LCIA method data set", "refObjectId": "b5c610fe-def3-11e6-bf01-fe55135034f3", "uri": "../lciamethods/b5c610fe-def3-11e6-bf01-fe55135034f3.xml"}, "other": {"anies": [{"name": "referenceToUnitGroupDataSet", "value": {"shortDescription": [{"value": "kg NMVOC eq", "lang": "en"}], "type": "unit group data set", "refObjectId": "d27c25f8-fbc1-44c6-b47b-4adbae4199c6", "uri": "../unitgroups/d27c25f8-fbc1-44c6-b47b-4adbae4199c6.xml"}}, {"value": "0.016602181570165", "module": "A1-A3"}, {"value": "2.23802621159091E-05", "module": "A4"}, {"value": "1.44068878891687E-05", "module": "A5"}, {"value": "1.18235914387535E-05", "module": "C1"}, {"value": "1.11901310579545E-05", "module": "C2"}, {"value": "0.00471383152622995", "module": "C3"}, {"value": "0", "module": "C4"}, {"value": "-0.00252266596833075", "module": "D"}]}}, {"referenceToLCIAMethodDataSet": {"shortDescription": [{"value": "Abiotic depletion potential for non fossil resources (ADPE)", "lang": "en"}, {"value": "Potenzial für den abiotischen Abbau nicht fossiler Ressourcen (ADPE)", "lang": "de"}], "type": "LCIA method data set", "refObjectId": "b2ad6494-c78d-11e6-9d9d-cec0c932ce01", "uri": "../lciamethods/b2ad6494-c78d-11e6-9d9d-cec0c932ce01.xml"}, "other": {"anies": [{"name": "referenceToUnitGroupDataSet", "value": {"shortDescription": [{"value": "kg Sb eq", "lang": "en"}], "type": "unit group data set", "refObjectId": "54ccd2d9-a32a-4fc2-923d-f2c8c93e89d4", "uri": "../unitgroups/54ccd2d9-a32a-4fc2-923d-f2c8c93e89d4.xml"}}, {"value": "5.75861632335906E-06", "module": "A1-A3"}, {"value": "2.0609688708228E-09", "module": "A4"}, {"value": "6.50413707438331E-10", "module": "A5"}, {"value": "7.71077400968588E-11", "module": "C1"}, {"value": "1.0304844354114E-09", "module": "C2"}, {"value": "1.29523972065359E-08", "module": "C3"}, {"value": "0", "module": "C4"}, {"value": "-3.81530671390391E-07", "module": "D"}]}}, {"referenceToLCIAMethodDataSet": {"shortDescription": [{"value": "Abiotic depletion potential for fossil resources (ADPF)", "lang": "en"}, {"value": "Potenzial für den abiotischen Abbau fossiler Brennstoffe (ADPF)", "lang": "de"}], "type": "LCIA method data set", "refObjectId": "b2ad6110-c78d-11e6-9d9d-cec0c932ce01", "uri": "../lciamethods/b2ad6110-c78d-11e6-9d9d-cec0c932ce01.xml"}, "other": {"anies": [{"name": "referenceToUnitGroupDataSet", "value": {"shortDescription": [{"value": "MJ", "lang": "en"}], "type": "unit group data set", "refObjectId": "93a60a57-a3c8-11da-a746-0800200c9a66", "uri": "../unitgroups/93a60a57-a3c8-11da-a746-0800200c9a66.xml"}}, {"value": "161.366826229649", "module": "A1-A3"}, {"value": "0.329460019671562", "module": "A4"}, {"value": "0.0552257426831889", "module": "A5"}, {"value": "0.0254846710414983", "module": "C1"}, {"value": "0.164730009835781", "module": "C2"}, {"value": "1.65730504042295", "module": "C3"}, {"value": "0", "module": "C4"}, {"value": "-42.9305135930331", "module": "D"}]}}, {"referenceToLCIAMethodDataSet": {"shortDescription": [{"value": "Water use (WDP)", "lang": "en"}, {"value": "Wassernutzung (WDP)", "lang": "de"}], "type": "LCIA method data set", "refObjectId": "b2ad66ce-c78d-11e6-9d9d-cec0c932ce01", "uri": "../lciamethods/b2ad66ce-c78d-11e6-9d9d-cec0c932ce01.xml"}, "other": {"anies": [{"name": "referenceToUnitGroupDataSet", "value": {"shortDescription": [{"value": "m^(3) world eq deprived", "lang": "en"}], "type": "unit group data set", "refObjectId": "6ae2df01-888e-46c8-b17d-49fa3869b476", "uri": "../unitgroups/6ae2df01-888e-46c8-b17d-49fa3869b476.xml"}}, {"value": "0.878578098730802", "module": "A1-A3"}, {"value": "0.000221139157504926", "module": "A4"}, {"value": "0.0141924249654118", "module": "A5"}, {"value": "3.50099752295495E-06", "module": "C1"}, {"value": "0.000110569578752463", "module": "C2"}, {"value": "0.633156498433805", "module": "C3"}, {"value": "0", "module": "C4"}, {"value": "-0.269548070764136", "module": "D"}]}}, {"referenceToLCIAMethodDataSet": {"shortDescription": [{"value": "Incidence of disease due to PM emissions (PM)", "lang": "en"}, {"value": "Auftreten von Krankheiten aufgrund von Feinstaubemissionen (PM)", "lang": "de"}], "type": "LCIA method data set", "refObjectId": "b5c602c6-def3-11e6-bf01-fe55135034f3", "uri": "../lciamethods/b5c602c6-def3-11e6-bf01-fe55135034f3.xml"}, "other": {"anies": [{"name": "referenceToUnitGroupDataSet", "value": {"shortDescription": [{"value": "Disease incidence", "lang": "en"}], "type": "unit group data set", "refObjectId": "3883559b-648f-4afc-8ba2-0bd24f3affa3", "uri": "../unitgroups/3883559b-648f-4afc-8ba2-0bd24f3affa3.xml"}}, {"value": "1.15986171077597E-07", "module": "A1-A3"}, {"value": "1.46651939286653E-10", "module": "A4"}, {"value": "2.27443786658259E-10", "module": "A5"}, {"value": "9.91149732064408E-11", "module": "C1"}, {"value": "7.33259696433269E-11", "module": "C2"}, {"value": "1.05124262758994E-08", "module": "C3"}, {"value": "0", "module": "C4"}, {"value": "-2.75423394534957E-08", "module": "D"}]}}, {"referenceToLCIAMethodDataSet": {"shortDescription": [{"value": "Human exposure efficiency relative to U235 (IR)", "lang": "en"}, {"value": "Wirkung durch Exposition des Menschen mit U235 (IR)", "lang": "de"}], "type": "LCIA method data set", "refObjectId": "b5c632be-def3-11e6-bf01-fe55135034f3", "uri": "../lciamethods/b5c632be-def3-11e6-bf01-fe55135034f3.xml"}, "other": {"anies": [{"name": "referenceToUnitGroupDataSet", "value": {"shortDescription": [{"value": "kBq U235 eq", "lang": "en"}], "type": "unit group data set", "refObjectId": "456b05bf-1415-44a9-9993-02452f554c09", "uri": "../unitgroups/456b05bf-1415-44a9-9993-02452f554c09.xml"}}, {"value": "0.283151867432094", "module": "A1-A3"}, {"value": "5.96067261478113E-05", "module": "A4"}, {"value": "0.000315509525583752", "module": "A5"}, {"value": "4.07516186120128E-06", "module": "C1"}, {"value": "2.98033630739057E-05", "module": "C2"}, {"value": "0.0109711293080117", "module": "C3"}, {"value": "0", "module": "C4"}, {"value": "-0.57394243794546", "module": "D"}]}}, {"referenceToLCIAMethodDataSet": {"shortDescription": [{"value": "Comparative toxic unit for ecosystems (ETP-fw)", "lang": "en"}, {"value": "Toxizitätsvergleichseinheit für Ökosysteme (ETP-fw)", "lang": "de"}], "type": "LCIA method data set", "refObjectId": "ee1082d1-b0f7-43ca-a1f0-21e2a4a74511", "uri": "../lciamethods/ee1082d1-b0f7-43ca-a1f0-21e2a4a74511.xml"}, "other": {"anies": [{"name": "referenceToUnitGroupDataSet", "value": {"shortDescription": [{"value": "CTUe", "lang": "en"}], "type": "unit group data set", "refObjectId": "aa959ded-f1eb-4efb-9c5c-2d60be36b3e6", "uri": "../unitgroups/aa959ded-f1eb-4efb-9c5c-2d60be36b3e6.xml"}}, {"value": "59.7971161296784", "module": "A1-A3"}, {"value": "0.228728860754396", "module": "A4"}, {"value": "0.0395280023411049", "module": "A5"}, {"value": "0.0177462404154727", "module": "C1"}, {"value": "0.114364430377198", "module": "C2"}, {"value": "0.565600126819069", "module": "C3"}, {"value": "0", "module": "C4"}, {"value": "-9.44866444647355", "module": "D"}]}}, {"referenceToLCIAMethodDataSet": {"shortDescription": [{"value": "Comparative toxic unit for humans (carcinogenic) (HTP-c)", "lang": "en"}, {"value": "Toxizitätsvergleichseinheit für Menschen (krebserregend) (HTP-c)", "lang": "de"}], "type": "LCIA method data set", "refObjectId": "2299222a-bbd8-474f-9d4f-4dd1f18aea7c", "uri": "../lciamethods/2299222a-bbd8-474f-9d4f-4dd1f18aea7c.xml"}, "other": {"anies": [{"name": "referenceToUnitGroupDataSet", "value": {"shortDescription": [{"value": "CTUh", "lang": "en"}], "type": "unit group data set", "refObjectId": "d4c9523e-2d7e-49fd-8469-998f547d3a70", "uri": "../unitgroups/d4c9523e-2d7e-49fd-8469-998f547d3a70.xml"}}, {"value": "2.73101060894998E-09", "module": "A1-A3"}, {"value": "4.61024118164735E-12", "module": "A4"}, {"value": "2.21551612443376E-12", "module": "A5"}, {"value": "3.28216024792944E-13", "module": "C1"}, {"value": "2.30512059082367E-12", "module": "C2"}, {"value": "4.27606504681438E-11", "module": "C3"}, {"value": "0", "module": "C4"}, {"value": "-4.33302166275592E-10", "module": "D"}]}}, {"referenceToLCIAMethodDataSet": {"shortDescription": [{"value": "Comparative toxic unit for humans (noncarcinogenic) (HTP-nc)", "lang": "en"}, {"value": "Toxizitätsvergleichseinheit für Menschen (nicht krebserregend) (HTP-nc)", "lang": "de"}], "type": "LCIA method data set", "refObjectId": "3af763a5-b7a1-48c9-9cee-1f223481fcef", "uri": "../lciamethods/3af763a5-b7a1-48c9-9cee-1f223481fcef.xml"}, "other": {"anies": [{"name": "referenceToUnitGroupDataSet", "value": {"shortDescription": [{"value": "CTUh", "lang": "en"}], "type": "unit group data set", "refObjectId": "d4c9523e-2d7e-49fd-8469-998f547d3a70", "uri": "../unitgroups/d4c9523e-2d7e-49fd-8469-998f547d3a70.xml"}}, {"value": "8.58691654184955E-08", "module": "A1-A3"}, {"value": "2.39229815316073E-10", "module": "A4"}, {"value": "2.24388771877397E-10", "module": "A5"}, {"value": "1.65935567222804E-11", "module": "C1"}, {"value": "1.19614907658036E-10", "module": "C2"}, {"value": "1.55113826785728E-09", "module": "C3"}, {"value": "0", "module": "C4"}, {"value": "-1.66388475334654E-08", "module": "D"}]}}, {"referenceToLCIAMethodDataSet": {"shortDescription": [{"value": "Soil quality index (SQP)", "lang": "en"}, {"value": "Bodenqualitätsindex (SQP)", "lang": "de"}], "type": "LCIA method data set", "refObjectId": "b2ad6890-c78d-11e6-9d9d-cec0c932ce01", "uri": "../lciamethods/b2ad6890-c78d-11e6-9d9d-cec0c932ce01.xml"}, "other": {"anies": [{"name": "referenceToUnitGroupDataSet", "value": {"shortDescription": [{"value": "SQP", "lang": "en"}], "type": "unit group data set", "refObjectId": "f130951c-e67f-4f7f-8dd4-665de3974e18", "uri": "../unitgroups/f130951c-e67f-4f7f-8dd4-665de3974e18.xml"}}, {"value": "10.7823349058433", "module": "A1-A3"}, {"value": "0.113366659012369", "module": "A4"}, {"value": "0.0141080092906318", "module": "A5"}, {"value": "7.03216191046978E-05", "module": "C1"}, {"value": "0.0566833295061845", "module": "C2"}, {"value": "0.347049481891671", "module": "C3"}, {"value": "0", "module": "C4"}, {"value": "-7.67665258635722", "module": "D"}]}}]}, "otherAttributes": {"{http://www.indata.network/EPD/2019}epd-version": "1.2"}, "version": "1.1", "locations": "../ILCDLocations.xml"}