{"processInformation": {"dataSetInformation": {"UUID": "3a523b2a-d2b1-4ef9-bdb5-9c13c9f6fcef", "name": {"baseName": [{"value": "Particleboard, coated", "lang": "en"}, {"value": "Spanplatte, melaminbeschichtet", "lang": "de"}], "functionalUnitFlowProperties": [{"lang": "en"}]}, "classificationInformation": {"classification": [{"class": [{"value": "Holz", "level": 0, "classId": "3"}, {"value": "Holzwerkstoffe", "level": 1, "classId": "3.2"}, {"value": "Spanplatten", "level": 2, "classId": "3.2.06"}], "name": "OEKOBAU.DAT"}, {"class": [{"value": "02 Building products", "level": 0}, {"value": "Wood based panels", "level": 1}, {"value": "Wood-based panels", "level": 2}], "name": "IBUCategories"}]}, "generalComment": [{"value": "Coated particleboard is a panel-shaped wood-based material in accordance with EN 312 and EN 14322, which is manufactured in a flat-pressing process by means of compression under heat of small wood particles with adhesive.\nDue to their various densities and adhesive systems, coated particleboards can display a variety of material properties and qualities like moisture resistance, fire-retardant or others.", "lang": "en"}, {"value": "Spanplatten sind plattenförmige Holzwerkstoffe nach EN 312 und EN 14322 sowie nach ANSI A208 für den nordamerikanischen Markt, die im Flachpressverfahren durch Verpressen von kleinen Holzpartikeln mit Klebstoff unter Hitzeeinwirkung hergestellt werden.\nAufgrund ihrer unterschiedlichen Dichten und Klebstoffsysteme können beschichtete Spanplatten eine Vielzahl von Materialeigenschaften und Qualitäten aufweisen, wie z.B. feuchtigkeitsbeständig, feuerhemmend oder andere.", "lang": "de"}]}, "quantitativeReference": {"referenceToReferenceFlow": [0]}, "time": {"referenceYear": 2024, "dataSetValidUntil": 2029, "other": {"anies": [{"name": "publicationDateOfEPD", "value": 1704844800000}]}}, "geography": {"locationOfOperationSupplyOrProduction": {"location": "RER"}}, "technology": {"technologyDescriptionAndIncludedProcesses": [{"value": "The wood is chipped, screened and dried. Surface layer and core layer materials are then glued and scattered on a forming belt as a particles’ mat. This is pressed into panels under high pressure in a hot press. The panels are trimmed, picked and sanded on both sides after cooling. Finaly the panels are coated with melamine impregnated paper in a short-cycle press. All leftovers incurred during board manufacture are redirected into the process or used as fuel to supply the energy needs of the manufacturing process on site. A process diagram is presented below. The production sites are certified according to the following standards: /ISO 9001:2008/; /ISO 14001:2009/; /OHSAS 18001:2007/; /EN ISO 50001:2011/ (German and Portuguese sites). \nDeclared unit: \nThe declared unit for the LCA is 1 m2 of average Sonae Arauco particleboard.", "lang": "en"}, {"value": "Das Holz wird zerkleinert, gesiebt und getrocknet. Anschließend werden Deckschicht- und Kernschichtmaterial verleimt und als Spänematte auf ein Formband gestreut. Diese wird unter hohem Druck in einer Heißpresse zu Platten gepresst. Nach dem Abkühlen werden die Platten auf beiden Seiten besäumt, gerupft und geschliffen.\nAbschließend werden die Platten in einer Kurztaktpresse mit melaminimprägniertem Papier beschichtet.\n\nAlle bei der Plattenherstellung anfallenden Reste werden in den Prozess zurückgeführt oder als Brennstoff zur Deckung des Energiebedarfs für den Herstellungsprozess vor Ort verwendet. \nTechnische Daten: \nsiehe die pdf datentabelle \nDeklarierte Einheit: \nDie deklarierte Einheit für die Ökobilanz ist 1 m2 einer durchschnittlichen Spanplatte von Sonae Arauco.\nDer gewichtete Durchschnitt wurde auf der Grundlage der Produktionsmengen der Werke in allen Ländern berechnet, in denen Sonae Arauco im Jahr 2021 tätig war (einige Werke 2020).", "lang": "de"}], "technologicalApplicability": [{"value": "The area of application for coated particleboard primarily involves decorative interior furnishings and furniture manufacturing.\nParticleboard can be classified into the following use classes according to the requirements\nestablished in EN 312:\nP1 General purpose boards for use in dry conditions\nP2 Boards for interior fitments (including furniture) for use in dry conditions\nP3 Non load-bearing boards for use in humid conditions\nP4 Load-bearing boards for use in dry conditions\nP5 Load-bearing boards for use in humid conditions\nP6 Heavy duty load-bearing boards for use in dry conditions\nP7 Heavy duty load-bearing boards for use in humid conditions", "lang": "en"}, {"value": "Der Anwendungsbereich für beschichtete Spanplatten liegt vor allem im dekorativen Innenausbau und\nInnenausbau und Möbelherstellung.\nSpanplatten können entsprechend den Anforderungen in folgende Verwendungsklassen eingeteilt werden\ndie in EN 312 festgelegt sind:\nP1 Platten für allgemeine Zwecke zur Verwendung unter trockenen Bedingungen\nP2 Platten für den Innenausbau (einschließlich Möbel) zur Verwendung unter trockenen Bedingungen\nP3 Nicht tragende Platten für die Verwendung in feuchten Umgebungen\nP4 Tragende Platten für die Verwendung unter trockenen Bedingungen\nP5 Tragende Platten für die Verwendung unter feuchten Bedingungen\nP6 Tragende Bretter für hohe Beanspruchung zur Verwendung unter trockenen Bedingungen\nP7 Schwerlast-Tragplatten für den Einsatz unter feuchten Bedingungen\nZusätzlich definiert die Klassifizierung nach ANSI A208.1 die folgenden Klassen:\nM1, MS Mitteldichte Handelsklasse\nM2, M3i Mitteldichte Industriequalität", "lang": "de"}]}}, "modellingAndValidation": {"LCIMethodAndAllocation": {"typeOfDataSet": "EPD", "referenceToLCAMethodDetails": [{"shortDescription": [{"value": "Wood-based panels.pdf", "lang": "en"}], "type": "source data set", "refObjectId": "6898d008-fa0b-4cac-a8e6-a553330ebd2a"}], "other": {"anies": [{"name": "subType", "value": "specific dataset"}]}}, "dataSourcesTreatmentAndRepresentativeness": {"referenceToDataSource": [{"shortDescription": [{"value": "ecoinvent database (all versions)", "lang": "en"}], "type": "source data set", "refObjectId": "b497a91f-e14b-4b69-8f28-f50eb1576766"}, {"shortDescription": [{"value": "ecoinvent 3.8 database", "lang": "en"}], "type": "source data set", "refObjectId": "0f4c65c0-6210-450f-b886-82bf8dd5ace9"}], "useAdviceForDataSet": [{"value": "Scope: \nThis document refers toparticleboard, coated with melamine-impregnated paper, manufactured in the following plants of the Sonae Arauco group:\nSonae Arauco Beeskow GmbH, Radinkendorfer Strasse 71, 15848 Beeskow, Germany\nSonae Arauco Deutschland GmbH - Nettgau Plant, Strohmweg 1, 38489 Nettgau, Germany\nSonae Arauco Portugal, SA, Estrada Nacional 17, n 59 e 61, 3400-691 S.Paio de Gramaas (Oliveira do Hospital), Portugal\nSonae Arauco South Africa (Pty) Ltd, Heidelberg Road, Rocky Drift, White River, Republic of South Africa\nSonae Arauco Espaa- Soluciones de Madera, S.L., Carretera Crdoba-Valencia Km 126, Estacin Linares-Baeza, 23490 Linares (Jan), Spain\nThe production volume of these plants covers 100 % of the total production of particleboard by the Sonae Arauco group. \nSystem boundary: \nType of the EPD: cradle-to-gate with modules C1 to C4 and module D (A1-A3, C and D)\n\nModules A1 – A3 of the production stage cover the manufacturing of the products, including raw material extraction and processing, energy generation, the production of ancillary products and packaging materials, transport, as well as all waste treatment processes. Eventual benefits of recycling or energy recovery are neglected.\n\nThe resource aspects of wood were inventoried via material inherent properties such as resource extraction of CO2 from the atmosphere and the lower heating value as the use of renewable energy. Material inherent properties are subject to co-product allocation as ruled in EN 15804.\n\nModule A4 covers the transport of the product from the production site to the construction site by a lorry over a default distance of 460 km.\n\nModule A5 covers the transport of the packaging material from the construction site and its disposal. Default end-of-waste states for the packaging materials from the packed products at the construction site are defined in analogy for wastes occurring in modules A1-A3. Eventual further inputs for the installation of the products are not considered due to the broad applicability of the assessed products.\nThe substituted primary material from the net amount of recycled material and from recovered energy exported from the product system in Module A5 is declared in Module D.\n\nModule C1 manual deconstruction isassumed. The declared values are thus 0.\n\nModule C2 includes the transport of the de-constructed product to a recycling centre by over 50 km.\n\nModule C3 covers the preparation of the post-consumer board to become a secondary fuel; the end-of-waste status for recycled wood-based boards is defined as the point where they have been sorted and chipped, ready to be used as secondary fuels.\nIn line with EN 16485, the export of the biogenic carbon stored in the board, expressed in CO2-equivalent is also reported in module C3.\n\nModule C4 is not relevant for the assumed end-of-life scenario. The declared values are thus 0.\n\nModule D compiles all the benefits and burdens associated with the secondary fuels, secondary materials and exported energy leaving the production system in the modules A5 and C3. Therefore, module D covers the avoided burdens from recycling and from energy recovered from the waste treatment in module A5 as well as the transport of the obsolete boards to a biomass combustion plant, the combustion process itself and the loads and benefits of the substitution of fossil fuels and/or electricity.\nSubstitution effects in module D are always calculated for the net amount of secondary material or secondary fuel of the product system in line with EN 16485.", "lang": "en"}, {"value": "Gültigkeitsbereich: \nDieses Dokument bezieht sich auf Spanplatten, beschichtet mit m\nelaminimprägniertem Papier, hergestellt in den folgenden Werken der Sonae Arauco Gruppe:\nSonae Arauco Beeskow GmbH, Radinkendorfer Straße 71, 15848 Beeskow, Deutschland\nSonae Arauco Deutschland GmbH - Werk Nettgau, Strohmweg 1, 38489 Nettgau, Deutschland\nSonae Arauco Portugal, SA, Quinta da Poça - S.Paio de Gramaços, 3404-954 Oliveira do Hospital, Portugal\nSonae Arauco South Africa (Pty) Ltd, White River, Südafrika\nSonae Arauco España- Soluciones de Madera, S.L., Carretera Córdoba-Valencia Km 126, Estación Linares-Baeza, 23490 Linares (Jaén), Spanien\nSonae Arauco España-Soluciones de Madera, S.L., Calle de Los Titulos, 29, 47009 Valladolid, Spanien\nDas Produktionsvolumen dieser Werke deckt 100 % der gesamten Spanplattenproduktion der Sonae Arauco Gruppe ab. \nSystemgrenze: \nModule A1-A3, A4, A5, C1, C2, C3, C3, D", "lang": "de"}], "other": {"anies": [{"name": "referenceToOriginalEPD", "value": {"shortDescription": {"value": "Particleboard, coated.pdf", "defaultValue": "Particleboard, coated.pdf", "lstrings": [{"lang": "en", "value": "Particleboard, coated.pdf"}]}, "type": "source data set", "uuid": {"uuid": "1f3b4548-6ae6-42d1-9514-1ce7f76260c8"}, "refObjectId": "1f3b4548-6ae6-42d1-9514-1ce7f76260c8", "resourceURLs": ["https://oekobaudat.de/OEKOBAU.DAT/resource/sources/1f3b4548-6ae6-42d1-9514-1ce7f76260c8/Particleboard_coated_19956.pdf?version=00.02.000"]}}]}}, "validation": {"review": [{"referenceToNameOfReviewerAndInstitution": [{"shortDescription": [{"value": "Institut Bauen und Umwelt e. V.", "lang": "en"}], "type": "contact data set", "refObjectId": "d111dbec-b024-4be5-86c5-752d6eb2cf95", "uri": "../contacts/d111dbec-b024-4be5-86c5-752d6eb2cf95.xml"}], "type": "Accredited third party review"}]}, "complianceDeclarations": {"compliance": [{"referenceToComplianceSystem": {"shortDescription": [{"value": "DIN EN 15804+A2", "lang": "en"}], "type": "source data set", "refObjectId": "c0016b33-8cf7-415c-ac6e-deba0d21440d", "uri": "../sources/c0016b33-8cf7-415c-ac6e-deba0d21440d.xml"}}, {"referenceToComplianceSystem": {"shortDescription": [{"value": "ISO 14025", "lang": "en"}], "type": "source data set", "refObjectId": "4f2eb655-6e44-4874-a95a-e28f5442cd4d", "uri": "../sources/4f2eb655-6e44-4874-a95a-e28f5442cd4d.xml"}}]}}, "administrativeInformation": {"commissionerAndGoal": {"referenceToCommissioner": [{"shortDescription": [{"value": "Sonae Arauco, S.A.", "lang": "en"}], "type": "contact data set", "refObjectId": "5aac1fae-fb0e-4257-9068-5d80fe2395e6", "uri": "../contacts/5aac1fae-fb0e-4257-9068-5d80fe2395e6.xml"}]}, "dataGenerator": {"referenceToPersonOrEntityGeneratingTheDataSet": [{"shortDescription": [{"value": "Dr. Frank Werner - Umwelt & Entwicklung", "lang": "en"}], "type": "contact data set", "refObjectId": "62792478-795c-4ae2-ac9a-1012d9515424", "uri": "../contacts/62792478-795c-4ae2-ac9a-1012d9515424.xml"}]}, "dataEntryBy": {"timeStamp": 1704844800000, "referenceToDataSetFormat": [{"shortDescription": [{"value": "ILCD Format", "lang": "en"}], "type": "source data set", "refObjectId": "a97a0155-0234-4b87-b4ce-a45da52f2a40", "uri": "../sources/a97a0155-0234-4b87-b4ce-a45da52f2a40.xml"}, {"shortDescription": [{"value": "EPD-Datenformaterweiterungen v1.2", "lang": "de"}, {"value": "EPD Data Format Extensions v1.2", "lang": "en"}], "type": "source data set", "refObjectId": "a29449fd-aa2f-4de8-b5d7-4b06b43c6fde", "uri": "../sources/a29449fd-aa2f-4de8-b5d7-4b06b43c6fde.xml"}]}, "publicationAndOwnership": {"dataSetVersion": "00.03.000", "referenceToRegistrationAuthority": {"shortDescription": [{"value": "Institut Bauen und Umwelt e. V.", "lang": "en"}], "type": "contact data set", "refObjectId": "d111dbec-b024-4be5-86c5-752d6eb2cf95", "uri": "../contacts/d111dbec-b024-4be5-86c5-752d6eb2cf95.xml"}, "registrationNumber": "EPD-SON-20230516-IBA2-EN", "referenceToOwnershipOfDataSet": {"shortDescription": [{"value": "Sonae Arauco, S.A.", "lang": "en"}], "type": "contact data set", "refObjectId": "5aac1fae-fb0e-4257-9068-5d80fe2395e6", "uri": "../contacts/5aac1fae-fb0e-4257-9068-5d80fe2395e6.xml"}, "copyright": true, "licenseType": "Free of charge for all users and uses", "accessRestrictions": [{"value": "None", "lang": "en"}], "other": {"anies": [{"name": "referenceToPublisher", "value": {"shortDescription": [{"value": "Institut Bauen und Umwelt e. V.", "lang": "en"}], "type": "contact data set", "refObjectId": "d111dbec-b024-4be5-86c5-752d6eb2cf95", "uri": "../contacts/d111dbec-b024-4be5-86c5-752d6eb2cf95.xml"}}]}}}, "exchanges": {"exchange": [{"dataSetInternalID": 0, "referenceToFlowDataSet": {"shortDescription": [{"value": "Particleboard, coated with melamine impregnated paper, per m² (Spanplatte, melaminbeschichtet)", "lang": "en"}], "type": "flow data set", "refObjectId": "dd0bfc88-e9be-15d5-a863-2f1dba417932", "uri": "../flows/dd0bfc88-e9be-15d5-a863-2f1dba417932.xml"}, "meanAmount": 1.0, "referencesToDataSource": {}, "referenceFlow": true, "resolvedFlowVersion": "00.03.000", "resultingflowAmount": 1.0, "flowProperties": [{"name": [{"lang": "de", "value": "Fläche"}, {"lang": "en", "value": "Area"}], "uuid": "93a60a56-a3c8-19da-a746-0800200c9a66", "referenceFlowProperty": true, "meanValue": 1.0, "referenceUnit": "qm", "unitGroupUUID": "c20a03d7-bd90-4569-bc94-66cfd364dfc8"}], "materialProperties": [{"name": "grammage", "value": "11.1", "unit": "kg/m^2", "unitDescription": "kilograms per square meter"}, {"name": "layer thickness", "value": "0.165", "unit": "m", "unitDescription": "meters"}, {"name": "gross density", "value": "650.0", "unit": "kg/m^3", "unitDescription": "kilograms per cubic metre"}], "typeOfFlow": "Product flow", "classification": {"classHierarchy": "Holz / Holzwerkstoffe / Spanplatten", "name": "OEKOBAU.DAT"}}, {"dataSetInternalID": 1, "referenceToFlowDataSet": {"shortDescription": [{"value": "Renewable primary energy as energy carrier (PERE)", "lang": "en"}, {"value": "Erneuerbare Primärenergie als Energieträger (PERE)", "lang": "de"}], "type": "flow data set", "refObjectId": "20f32be5-0398-4288-9b6d-accddd195317", "uri": "../flows/20f32be5-0398-4288-9b6d-accddd195317.xml"}, "exchange direction": "INPUT", "other": {"anies": [{"name": "referenceToUnitGroupDataSet", "value": {"shortDescription": [{"value": "MJ", "lang": "en"}], "type": "unit group data set", "refObjectId": "93a60a57-a3c8-11da-a746-0800200c9a66", "uri": "../unitgroups/93a60a57-a3c8-11da-a746-0800200c9a66.xml"}}, {"value": "-99.9332009168696", "module": "A1-A3"}, {"value": "0.179180096977214", "module": "A4"}, {"value": "2.14076384355449", "module": "A5"}, {"value": "0", "module": "C1"}, {"value": "0.0294775255843193", "module": "C2"}, {"value": "0.35573820932627", "module": "C3"}, {"value": "0", "module": "C4"}, {"value": "-5.13368579376348", "module": "D"}]}, "resolvedFlowVersion": "38.00.000", "flowProperties": [], "typeOfFlow": "Other flow", "classification": {"classHierarchy": "Quantities", "name": "GaBiCategories"}}, {"dataSetInternalID": 2, "referenceToFlowDataSet": {"shortDescription": [{"value": "Renewable primary energy resources as material utilization (PERM)", "lang": "en"}, {"value": "Erneuerbare Primärenergie zur stofflichen Nutzung (PERM)", "lang": "de"}], "type": "flow data set", "refObjectId": "fb3ec0de-548d-4508-aea5-00b73bf6f702", "uri": "../flows/fb3ec0de-548d-4508-aea5-00b73bf6f702.xml"}, "exchange direction": "INPUT", "other": {"anies": [{"name": "referenceToUnitGroupDataSet", "value": {"shortDescription": [{"value": "MJ", "lang": "en"}], "type": "unit group data set", "refObjectId": "93a60a57-a3c8-11da-a746-0800200c9a66", "uri": "../unitgroups/93a60a57-a3c8-11da-a746-0800200c9a66.xml"}}, {"value": "173.14", "module": "A1-A3"}, {"value": "0", "module": "A4"}, {"value": "-2.14", "module": "A5"}, {"value": "0", "module": "C1"}, {"value": "0", "module": "C2"}, {"value": "-171", "module": "C3"}, {"value": "0", "module": "C4"}, {"value": "0", "module": "D"}]}, "resolvedFlowVersion": "38.00.000", "flowProperties": [], "typeOfFlow": "Other flow", "classification": {"classHierarchy": "Quantities", "name": "GaBiCategories"}}, {"dataSetInternalID": 3, "referenceToFlowDataSet": {"shortDescription": [{"value": "Total use of renewable primary energy resources (PERT)", "lang": "en"}, {"value": "Total erneuerbare Primärenergie (PERT)", "lang": "de"}], "type": "flow data set", "refObjectId": "53f97275-fa8a-4cdd-9024-65936002acd0", "uri": "../flows/53f97275-fa8a-4cdd-9024-65936002acd0.xml"}, "exchange direction": "INPUT", "other": {"anies": [{"name": "referenceToUnitGroupDataSet", "value": {"shortDescription": [{"value": "MJ", "lang": "en"}], "type": "unit group data set", "refObjectId": "93a60a57-a3c8-11da-a746-0800200c9a66", "uri": "../unitgroups/93a60a57-a3c8-11da-a746-0800200c9a66.xml"}}, {"value": "73.2067990831304", "module": "A1-A3"}, {"value": "0.179180096977214", "module": "A4"}, {"value": "0.000763843554490245", "module": "A5"}, {"value": "0", "module": "C1"}, {"value": "0.0294775255843193", "module": "C2"}, {"value": "-170.644261790674", "module": "C3"}, {"value": "0", "module": "C4"}, {"value": "-5.13368579376348", "module": "D"}]}, "resolvedFlowVersion": "38.00.000", "flowProperties": [], "typeOfFlow": "Other flow", "classification": {"classHierarchy": "Quantities / Environmental quantities / EPD EN 15804 / LCI indicators", "name": "GaBiCategories"}}, {"dataSetInternalID": 4, "referenceToFlowDataSet": {"shortDescription": [{"value": "Non renewable primary energy as energy carrier (PENRE)", "lang": "en"}, {"value": "Nicht-erneuerbare Primärenergie als Energieträger (PENRE)", "lang": "de"}], "type": "flow data set", "refObjectId": "ac857178-2b45-46ec-892a-a9a4332f0372", "uri": "../flows/ac857178-2b45-46ec-892a-a9a4332f0372.xml"}, "exchange direction": "INPUT", "other": {"anies": [{"name": "referenceToUnitGroupDataSet", "value": {"shortDescription": [{"value": "MJ", "lang": "en"}], "type": "unit group data set", "refObjectId": "93a60a57-a3c8-11da-a746-0800200c9a66", "uri": "../unitgroups/93a60a57-a3c8-11da-a746-0800200c9a66.xml"}}, {"value": "121.79849110492", "module": "A1-A3"}, {"value": "12.7766458115477", "module": "A4"}, {"value": "0.173291163968583", "module": "A5"}, {"value": "0", "module": "C1"}, {"value": "1.77404601237153", "module": "C2"}, {"value": "2.06562262408933", "module": "C3"}, {"value": "0", "module": "C4"}, {"value": "-153.763256869597", "module": "D"}]}, "resolvedFlowVersion": "38.00.000", "flowProperties": [], "typeOfFlow": "Other flow", "classification": {"classHierarchy": "Quantities", "name": "GaBiCategories"}}, {"dataSetInternalID": 5, "referenceToFlowDataSet": {"shortDescription": [{"value": "Non renewable primary energy as material utilization (PENRM)", "lang": "en"}, {"value": "Nicht-erneuerbare Primärenergie zur stofflichen Nutzung (PENRM)", "lang": "de"}], "type": "flow data set", "refObjectId": "1421caa0-679d-4bf4-b282-0eb850ccae27", "uri": "../flows/1421caa0-679d-4bf4-b282-0eb850ccae27.xml"}, "exchange direction": "INPUT", "other": {"anies": [{"name": "referenceToUnitGroupDataSet", "value": {"shortDescription": [{"value": "MJ", "lang": "en"}], "type": "unit group data set", "refObjectId": "93a60a57-a3c8-11da-a746-0800200c9a66", "uri": "../unitgroups/93a60a57-a3c8-11da-a746-0800200c9a66.xml"}}, {"value": "27.306", "module": "A1-A3"}, {"value": "0", "module": "A4"}, {"value": "-0.106", "module": "A5"}, {"value": "0", "module": "C1"}, {"value": "0", "module": "C2"}, {"value": "-27.2", "module": "C3"}, {"value": "0", "module": "C4"}, {"value": "0", "module": "D"}]}, "resolvedFlowVersion": "38.00.000", "flowProperties": [], "typeOfFlow": "Other flow", "classification": {"classHierarchy": "Quantities", "name": "GaBiCategories"}}, {"dataSetInternalID": 6, "referenceToFlowDataSet": {"shortDescription": [{"value": "Total use of non renewable primary energy resources (PENRT)", "lang": "en"}, {"value": "Total nicht erneuerbare Primärenergie (PENRT)", "lang": "de"}], "type": "flow data set", "refObjectId": "06159210-646b-4c8d-8583-da9b3b95a6c1", "uri": "../flows/06159210-646b-4c8d-8583-da9b3b95a6c1.xml"}, "exchange direction": "INPUT", "other": {"anies": [{"name": "referenceToUnitGroupDataSet", "value": {"shortDescription": [{"value": "MJ", "lang": "en"}], "type": "unit group data set", "refObjectId": "93a60a57-a3c8-11da-a746-0800200c9a66", "uri": "../unitgroups/93a60a57-a3c8-11da-a746-0800200c9a66.xml"}}, {"value": "149.10449110492", "module": "A1-A3"}, {"value": "12.7766458115477", "module": "A4"}, {"value": "0.067291163968583", "module": "A5"}, {"value": "0", "module": "C1"}, {"value": "1.77404601237153", "module": "C2"}, {"value": "-25.1343773759107", "module": "C3"}, {"value": "0", "module": "C4"}, {"value": "-153.763256869597", "module": "D"}]}, "resolvedFlowVersion": "38.00.000", "flowProperties": [], "typeOfFlow": "Other flow", "classification": {"classHierarchy": "Quantities / Environmental quantities / EPD EN 15804 / LCI indicators", "name": "GaBiCategories"}}, {"dataSetInternalID": 7, "referenceToFlowDataSet": {"shortDescription": [{"value": "Use of secondary material (SM)", "lang": "en"}, {"value": "Einsatz von Sekundärstoffen (SM)", "lang": "de"}], "type": "flow data set", "refObjectId": "c6a1f35f-2d09-4f54-8dfb-97e502e1ce92", "uri": "../flows/c6a1f35f-2d09-4f54-8dfb-97e502e1ce92.xml"}, "exchange direction": "INPUT", "other": {"anies": [{"name": "referenceToUnitGroupDataSet", "value": {"shortDescription": [{"value": "kg", "lang": "en"}], "type": "unit group data set", "refObjectId": "ad38d542-3fe9-439d-9b95-2f5f7752acaf", "uri": "../unitgroups/ad38d542-3fe9-439d-9b95-2f5f7752acaf.xml"}}, {"value": "2.69353506427316", "module": "A1-A3"}, {"value": "0", "module": "A4"}, {"value": "0", "module": "A5"}, {"value": "0", "module": "C1"}, {"value": "0", "module": "C2"}, {"value": "0", "module": "C3"}, {"value": "0", "module": "C4"}, {"value": "0", "module": "D"}]}, "resolvedFlowVersion": "38.00.000", "flowProperties": [], "typeOfFlow": "Other flow", "classification": {"classHierarchy": "Quantities / Environmental quantities / EPD EN 15804 / LCI indicators", "name": "GaBiCategories"}}, {"dataSetInternalID": 8, "referenceToFlowDataSet": {"shortDescription": [{"value": "Use of renewable secondary fuels (RSF)", "lang": "en"}, {"value": "Erneuerbare Sekundärbrennstoffe (RSF)", "lang": "de"}], "type": "flow data set", "refObjectId": "64333088-a55f-4aa2-9a31-c10b07816787", "uri": "../flows/64333088-a55f-4aa2-9a31-c10b07816787.xml"}, "exchange direction": "INPUT", "other": {"anies": [{"name": "referenceToUnitGroupDataSet", "value": {"shortDescription": [{"value": "MJ", "lang": "en"}], "type": "unit group data set", "refObjectId": "93a60a57-a3c8-11da-a746-0800200c9a66", "uri": "../unitgroups/93a60a57-a3c8-11da-a746-0800200c9a66.xml"}}, {"value": "69.1883283625075", "module": "A1-A3"}, {"value": "0", "module": "A4"}, {"value": "0", "module": "A5"}, {"value": "0", "module": "C1"}, {"value": "0", "module": "C2"}, {"value": "0", "module": "C3"}, {"value": "0", "module": "C4"}, {"value": "105.157164042728", "module": "D"}]}, "resolvedFlowVersion": "38.00.000", "flowProperties": [], "typeOfFlow": "Other flow", "classification": {"classHierarchy": "Quantities / Environmental quantities / EPD EN 15804 / LCI indicators", "name": "GaBiCategories"}}, {"dataSetInternalID": 9, "referenceToFlowDataSet": {"shortDescription": [{"value": "Use of non renewable secondary fuels (NRSF)", "lang": "en"}, {"value": "Nicht erneuerbare Sekundärbrennstoffe (NRSF)", "lang": "de"}], "type": "flow data set", "refObjectId": "89def144-d39a-4287-b86f-efde453ddcb2", "uri": "../flows/89def144-d39a-4287-b86f-efde453ddcb2.xml"}, "exchange direction": "INPUT", "other": {"anies": [{"name": "referenceToUnitGroupDataSet", "value": {"shortDescription": [{"value": "MJ", "lang": "en"}], "type": "unit group data set", "refObjectId": "93a60a57-a3c8-11da-a746-0800200c9a66", "uri": "../unitgroups/93a60a57-a3c8-11da-a746-0800200c9a66.xml"}}, {"value": "0", "module": "A1-A3"}, {"value": "0", "module": "A4"}, {"value": "0", "module": "A5"}, {"value": "0", "module": "C1"}, {"value": "0", "module": "C2"}, {"value": "0", "module": "C3"}, {"value": "0", "module": "C4"}, {"value": "33.6652295783312", "module": "D"}]}, "resolvedFlowVersion": "38.00.000", "flowProperties": [], "typeOfFlow": "Other flow", "classification": {"classHierarchy": "Quantities / Environmental quantities / EPD EN 15804 / LCI indicators", "name": "GaBiCategories"}}, {"dataSetInternalID": 10, "referenceToFlowDataSet": {"shortDescription": [{"value": "Use of net fresh water (FW)", "lang": "en"}, {"value": "Einsatz von Süßwasserressourcen (FW)", "lang": "de"}], "type": "flow data set", "refObjectId": "3cf952c8-f3a4-461d-8c96-96456ca62246", "uri": "../flows/3cf952c8-f3a4-461d-8c96-96456ca62246.xml"}, "exchange direction": "INPUT", "other": {"anies": [{"name": "referenceToUnitGroupDataSet", "value": {"shortDescription": [{"value": "m^3", "lang": "en"}], "type": "unit group data set", "refObjectId": "cd950537-0a98-4044-9ba7-9f9a68d0a504", "uri": "../unitgroups/cd950537-0a98-4044-9ba7-9f9a68d0a504.xml"}}, {"value": "0.215148693672609", "module": "A1-A3"}, {"value": "0.00135237124615983", "module": "A4"}, {"value": "5.67029756485959E-05", "module": "A5"}, {"value": "0", "module": "C1"}, {"value": "5.67029756485959E-05", "module": "C2"}, {"value": "0.00125051624899657", "module": "C3"}, {"value": "0", "module": "C4"}, {"value": "-0.0117943573511479", "module": "D"}]}, "resolvedFlowVersion": "38.00.000", "flowProperties": [], "typeOfFlow": "Other flow", "classification": {"classHierarchy": "Quantities / Environmental quantities / EPD EN 15804 / LCI indicators", "name": "GaBiCategories"}}, {"dataSetInternalID": 11, "referenceToFlowDataSet": {"shortDescription": [{"value": "Hazardous waste disposed (HWD)", "lang": "en"}, {"value": "Gefährlicher Abfall zur Deponie (HWD)", "lang": "de"}], "type": "flow data set", "refObjectId": "430f9e0f-59b2-46a0-8e0d-55e0e84948fc", "uri": "../flows/430f9e0f-59b2-46a0-8e0d-55e0e84948fc.xml"}, "exchange direction": "OUTPUT", "other": {"anies": [{"name": "referenceToUnitGroupDataSet", "value": {"shortDescription": [{"value": "kg", "lang": "en"}], "type": "unit group data set", "refObjectId": "ad38d542-3fe9-439d-9b95-2f5f7752acaf", "uri": "../unitgroups/ad38d542-3fe9-439d-9b95-2f5f7752acaf.xml"}}, {"value": "0.000207425087144014", "module": "A1-A3"}, {"value": "3.33434703125733E-05", "module": "A4"}, {"value": "5.3375296908157E-08", "module": "A5"}, {"value": "0", "module": "C1"}, {"value": "4.75006464923072E-06", "module": "C2"}, {"value": "9.52249896833877E-07", "module": "C3"}, {"value": "0", "module": "C4"}, {"value": "-0.000166501227836863", "module": "D"}]}, "resolvedFlowVersion": "38.00.000", "flowProperties": [], "typeOfFlow": "Other flow", "classification": {"classHierarchy": "Quantities / Environmental quantities / EPD EN 15804 / LCI indicators", "name": "GaBiCategories"}}, {"dataSetInternalID": 12, "referenceToFlowDataSet": {"shortDescription": [{"value": "Non hazardous waste disposed (NHWD)", "lang": "en"}, {"value": "Entsorgter nicht gefährlicher Abfall (NHWD)", "lang": "de"}], "type": "flow data set", "refObjectId": "b29ef66b-e286-4afa-949f-62f1a7b4d7fa", "uri": "../flows/b29ef66b-e286-4afa-949f-62f1a7b4d7fa.xml"}, "exchange direction": "OUTPUT", "other": {"anies": [{"name": "referenceToUnitGroupDataSet", "value": {"shortDescription": [{"value": "kg", "lang": "en"}], "type": "unit group data set", "refObjectId": "ad38d542-3fe9-439d-9b95-2f5f7752acaf", "uri": "../unitgroups/ad38d542-3fe9-439d-9b95-2f5f7752acaf.xml"}}, {"value": "1.56949485729825", "module": "A1-A3"}, {"value": "0.670620474983627", "module": "A4"}, {"value": "0.00167396224280197", "module": "A5"}, {"value": "0", "module": "C1"}, {"value": "0.0759204541686729", "module": "C2"}, {"value": "0.0135509283200034", "module": "C3"}, {"value": "0", "module": "C4"}, {"value": "0.186223561162006", "module": "D"}]}, "resolvedFlowVersion": "38.00.000", "flowProperties": [], "typeOfFlow": "Other flow", "classification": {"classHierarchy": "Quantities / Environmental quantities / EPD EN 15804 / LCI indicators", "name": "GaBiCategories"}}, {"dataSetInternalID": 13, "referenceToFlowDataSet": {"shortDescription": [{"value": "Radioactive waste disposed (RWD)", "lang": "en"}, {"value": "Entsorgter radioaktiver Abfall (RWD)", "lang": "de"}], "type": "flow data set", "refObjectId": "3449546e-52ad-4b39-b809-9fb77cea8ff6", "uri": "../flows/3449546e-52ad-4b39-b809-9fb77cea8ff6.xml"}, "exchange direction": "OUTPUT", "other": {"anies": [{"name": "referenceToUnitGroupDataSet", "value": {"shortDescription": [{"value": "kg", "lang": "en"}], "type": "unit group data set", "refObjectId": "ad38d542-3fe9-439d-9b95-2f5f7752acaf", "uri": "../unitgroups/ad38d542-3fe9-439d-9b95-2f5f7752acaf.xml"}}, {"value": "0.000660446935806417", "module": "A1-A3"}, {"value": "0.000184827482575574", "module": "A4"}, {"value": "9.08844581407538E-07", "module": "A5"}, {"value": "0", "module": "C1"}, {"value": "2.54002200219466E-05", "module": "C2"}, {"value": "2.68441050052881E-05", "module": "C3"}, {"value": "0", "module": "C4"}, {"value": "-0.000481862946037429", "module": "D"}]}, "resolvedFlowVersion": "38.00.000", "flowProperties": [], "typeOfFlow": "Other flow", "classification": {"classHierarchy": "Quantities / Environmental quantities / EPD EN 15804 / LCI indicators", "name": "GaBiCategories"}}, {"dataSetInternalID": 14, "referenceToFlowDataSet": {"shortDescription": [{"value": "Components for re-use (CRU)", "lang": "en"}, {"value": "Komponenten für die Wiederverwendung (CRU)", "lang": "de"}], "type": "flow data set", "refObjectId": "a2b32f97-3fc7-4af2-b209-525bc6426f33", "uri": "../flows/a2b32f97-3fc7-4af2-b209-525bc6426f33.xml"}, "exchange direction": "OUTPUT", "other": {"anies": [{"name": "referenceToUnitGroupDataSet", "value": {"shortDescription": [{"value": "kg", "lang": "en"}], "type": "unit group data set", "refObjectId": "ad38d542-3fe9-439d-9b95-2f5f7752acaf", "uri": "../unitgroups/ad38d542-3fe9-439d-9b95-2f5f7752acaf.xml"}}, {"value": "0", "module": "A1-A3"}, {"value": "0", "module": "A4"}, {"value": "0", "module": "A5"}, {"value": "0", "module": "C1"}, {"value": "0", "module": "C2"}, {"value": "0", "module": "C3"}, {"value": "0", "module": "C4"}, {"value": "0", "module": "D"}]}, "resolvedFlowVersion": "38.00.000", "flowProperties": [], "typeOfFlow": "Other flow", "classification": {"classHierarchy": "Quantities / Environmental quantities / EPD EN 15804 / LCI indicators", "name": "GaBiCategories"}}, {"dataSetInternalID": 15, "referenceToFlowDataSet": {"shortDescription": [{"value": "Materials for recycling (MFR)", "lang": "en"}, {"value": "Stoffe zum Recycling (MFR)", "lang": "de"}], "type": "flow data set", "refObjectId": "d7fe48a5-4103-49c8-9aae-b0b5dfdbd6ae", "uri": "../flows/d7fe48a5-4103-49c8-9aae-b0b5dfdbd6ae.xml"}, "exchange direction": "OUTPUT", "other": {"anies": [{"name": "referenceToUnitGroupDataSet", "value": {"shortDescription": [{"value": "kg", "lang": "en"}], "type": "unit group data set", "refObjectId": "ad38d542-3fe9-439d-9b95-2f5f7752acaf", "uri": "../unitgroups/ad38d542-3fe9-439d-9b95-2f5f7752acaf.xml"}}, {"value": "0.0129317792076216", "module": "A1-A3"}, {"value": "0", "module": "A4"}, {"value": "0.00559005464239365", "module": "A5"}, {"value": "0", "module": "C1"}, {"value": "0", "module": "C2"}, {"value": "0", "module": "C3"}, {"value": "0", "module": "C4"}, {"value": "0", "module": "D"}]}, "resolvedFlowVersion": "38.00.000", "flowProperties": [], "typeOfFlow": "Other flow", "classification": {"classHierarchy": "Quantities / Environmental quantities / EPD EN 15804 / LCI indicators", "name": "GaBiCategories"}}, {"dataSetInternalID": 16, "referenceToFlowDataSet": {"shortDescription": [{"value": "Materials for energy recovery (MER)", "lang": "en"}, {"value": "Stoffe für die Energierückgewinnung (MER)", "lang": "de"}], "type": "flow data set", "refObjectId": "59a9181c-3aaf-46ee-8b13-2b3723b6e447", "uri": "../flows/59a9181c-3aaf-46ee-8b13-2b3723b6e447.xml"}, "exchange direction": "OUTPUT", "other": {"anies": [{"name": "referenceToUnitGroupDataSet", "value": {"shortDescription": [{"value": "kg", "lang": "en"}], "type": "unit group data set", "refObjectId": "ad38d542-3fe9-439d-9b95-2f5f7752acaf", "uri": "../unitgroups/ad38d542-3fe9-439d-9b95-2f5f7752acaf.xml"}}, {"value": "0", "module": "A1-A3"}, {"value": "0", "module": "A4"}, {"value": "0", "module": "A5"}, {"value": "0", "module": "C1"}, {"value": "0", "module": "C2"}, {"value": "12.0747684088239", "module": "C3"}, {"value": "0", "module": "C4"}, {"value": "0", "module": "D"}]}, "resolvedFlowVersion": "38.00.000", "flowProperties": [], "typeOfFlow": "Other flow", "classification": {"classHierarchy": "Quantities / Environmental quantities / EPD EN 15804 / LCI indicators", "name": "GaBiCategories"}}, {"dataSetInternalID": 17, "referenceToFlowDataSet": {"shortDescription": [{"value": "Exported electrical energy (EEE)", "lang": "en"}, {"value": "Exportierte elektrische Energie (EEE)", "lang": "de"}], "type": "flow data set", "refObjectId": "4da0c987-2b76-40d6-9e9e-82a017aaaf29", "uri": "../flows/4da0c987-2b76-40d6-9e9e-82a017aaaf29.xml"}, "exchange direction": "OUTPUT", "other": {"anies": [{"name": "referenceToUnitGroupDataSet", "value": {"shortDescription": [{"value": "MJ", "lang": "en"}], "type": "unit group data set", "refObjectId": "93a60a57-a3c8-11da-a746-0800200c9a66", "uri": "../unitgroups/93a60a57-a3c8-11da-a746-0800200c9a66.xml"}}, {"value": "0.000448079253467013", "module": "A1-A3"}, {"value": "0", "module": "A4"}, {"value": "0.0762615278391672", "module": "A5"}, {"value": "0", "module": "C1"}, {"value": "0", "module": "C2"}, {"value": "0", "module": "C3"}, {"value": "0", "module": "C4"}, {"value": "0", "module": "D"}]}, "resolvedFlowVersion": "38.00.000", "flowProperties": [], "typeOfFlow": "Other flow", "classification": {"classHierarchy": "Quantities / Environmental quantities / EPD EN 15804 / LCI indicators", "name": "GaBiCategories"}}, {"dataSetInternalID": 18, "referenceToFlowDataSet": {"shortDescription": [{"value": "Exported thermal energy (EET)", "lang": "en"}, {"value": "Exportierte thermische Energie (EET)", "lang": "de"}], "type": "flow data set", "refObjectId": "98daf38a-7a79-46d3-9a37-2b7bd0955810", "uri": "../flows/98daf38a-7a79-46d3-9a37-2b7bd0955810.xml"}, "exchange direction": "OUTPUT", "other": {"anies": [{"name": "referenceToUnitGroupDataSet", "value": {"shortDescription": [{"value": "MJ", "lang": "en"}], "type": "unit group data set", "refObjectId": "93a60a57-a3c8-11da-a746-0800200c9a66", "uri": "../unitgroups/93a60a57-a3c8-11da-a746-0800200c9a66.xml"}}, {"value": "0.00515291141487064", "module": "A1-A3"}, {"value": "0", "module": "A4"}, {"value": "0.877007570150423", "module": "A5"}, {"value": "0", "module": "C1"}, {"value": "0", "module": "C2"}, {"value": "0", "module": "C3"}, {"value": "0", "module": "C4"}, {"value": "0", "module": "D"}]}, "resolvedFlowVersion": "38.00.000", "flowProperties": [], "typeOfFlow": "Other flow", "classification": {"classHierarchy": "Quantities / Environmental quantities / EPD EN 15804 / LCI indicators", "name": "GaBiCategories"}}]}, "LCIAResults": {"LCIAResult": [{"referenceToLCIAMethodDataSet": {"shortDescription": [{"value": "Global Warming Potential total (GWP-total)", "lang": "en"}, {"value": "Globales Erwärmungspotenzial total (GWP-total)", "lang": "de"}], "type": "LCIA method data set", "refObjectId": "6a37f984-a4b3-458a-a20a-64418c145fa2", "uri": "../lciamethods/6a37f984-a4b3-458a-a20a-64418c145fa2.xml"}, "other": {"anies": [{"name": "referenceToUnitGroupDataSet", "value": {"shortDescription": [{"value": "kg CO_(2) eq", "lang": "en"}], "type": "unit group data set", "refObjectId": "1ebf3012-d0db-4de2-aefd-ef30cedb0be1", "uri": "../unitgroups/1ebf3012-d0db-4de2-aefd-ef30cedb0be1.xml"}}, {"value": "-9.11315838417776", "module": "A1-A3"}, {"value": "0.843061542335415", "module": "A4"}, {"value": "0.210592498414385", "module": "A5"}, {"value": "0", "module": "C1"}, {"value": "0.118485323082807", "module": "C2"}, {"value": "16.598522518867", "module": "C3"}, {"value": "0", "module": "C4"}, {"value": "-5.17239769598268", "module": "D"}]}}, {"referenceToLCIAMethodDataSet": {"shortDescription": [{"value": "Global Warming Potential fossil fuels (GWP-fossil)", "lang": "en"}, {"value": "Globales Erwärmungspotenzial fossil (GWP-fossil)", "lang": "de"}], "type": "LCIA method data set", "refObjectId": "5f635281-343e-44fb-83df-1971b155e6b6", "uri": "../lciamethods/5f635281-343e-44fb-83df-1971b155e6b6.xml"}, "other": {"anies": [{"name": "referenceToUnitGroupDataSet", "value": {"shortDescription": [{"value": "kg CO_(2) eq", "lang": "en"}], "type": "unit group data set", "refObjectId": "1ebf3012-d0db-4de2-aefd-ef30cedb0be1", "uri": "../unitgroups/1ebf3012-d0db-4de2-aefd-ef30cedb0be1.xml"}}, {"value": "7.57323318321248", "module": "A1-A3"}, {"value": "0.84272544644624", "module": "A4"}, {"value": "0.012591757995017", "module": "A5"}, {"value": "0", "module": "C1"}, {"value": "0.118429335528506", "module": "C2"}, {"value": "0.0982971710411665", "module": "C3"}, {"value": "0", "module": "C4"}, {"value": "-5.16917802660226", "module": "D"}]}}, {"referenceToLCIAMethodDataSet": {"shortDescription": [{"value": "Global Warming Potential biogenic (GWP-biogenic)", "lang": "en"}, {"value": "Globales Erwärmungspotenzial biogen (GWP-biogenic)", "lang": "de"}], "type": "LCIA method data set", "refObjectId": "2356e1ab-0185-4db5-86e5-16de51c7485c", "uri": "../lciamethods/2356e1ab-0185-4db5-86e5-16de51c7485c.xml"}, "other": {"anies": [{"name": "referenceToUnitGroupDataSet", "value": {"shortDescription": [{"value": "kg CO_(2) eq", "lang": "en"}], "type": "unit group data set", "refObjectId": "1ebf3012-d0db-4de2-aefd-ef30cedb0be1", "uri": "../unitgroups/1ebf3012-d0db-4de2-aefd-ef30cedb0be1.xml"}}, {"value": "-16.698", "module": "A1-A3"}, {"value": "0", "module": "A4"}, {"value": "0.198", "module": "A5"}, {"value": "0", "module": "C1"}, {"value": "0", "module": "C2"}, {"value": "16.5", "module": "C3"}, {"value": "0", "module": "C4"}, {"value": "0", "module": "D"}]}}, {"referenceToLCIAMethodDataSet": {"shortDescription": [{"value": "Global Warming Potential luluc (GWP-luluc)", "lang": "en"}, {"value": "Globales Erwärmungspotenzial luluc (GWP-luluc)", "lang": "de"}], "type": "LCIA method data set", "refObjectId": "4331bbdb-978a-490d-8707-eeb047f01a55", "uri": "../lciamethods/4331bbdb-978a-490d-8707-eeb047f01a55.xml"}, "other": {"anies": [{"name": "referenceToUnitGroupDataSet", "value": {"shortDescription": [{"value": "kg CO_(2) eq", "lang": "en"}], "type": "unit group data set", "refObjectId": "1ebf3012-d0db-4de2-aefd-ef30cedb0be1", "uri": "../unitgroups/1ebf3012-d0db-4de2-aefd-ef30cedb0be1.xml"}}, {"value": "0.0116084326097573", "module": "A1-A3"}, {"value": "0.000336095889175211", "module": "A4"}, {"value": "7.40419367900585E-07", "module": "A5"}, {"value": "0", "module": "C1"}, {"value": "5.59875543006968E-05", "module": "C2"}, {"value": "0.000225347825801515", "module": "C3"}, {"value": "0", "module": "C4"}, {"value": "-0.00321966938041903", "module": "D"}]}}, {"referenceToLCIAMethodDataSet": {"shortDescription": [{"value": "Depletion potential of the stratospheric ozone layer (ODP)", "lang": "en"}, {"value": "Abbau Potential der stratosphärischen Ozonschicht (ODP)", "lang": "de"}], "type": "LCIA method data set", "refObjectId": "b5c629d6-def3-11e6-bf01-fe55135034f3", "uri": "../lciamethods/b5c629d6-def3-11e6-bf01-fe55135034f3.xml"}, "other": {"anies": [{"name": "referenceToUnitGroupDataSet", "value": {"shortDescription": [{"value": "kg CFC11 eq", "lang": "en"}], "type": "unit group data set", "refObjectId": "d9e957c9-7309-4474-bf3a-7777df6c4e5b", "uri": "../unitgroups/d9e957c9-7309-4474-bf3a-7777df6c4e5b.xml"}}, {"value": "1.08104985671458E-06", "module": "A1-A3"}, {"value": "1.95253291829661E-07", "module": "A4"}, {"value": "1.04952774812122E-09", "module": "A5"}, {"value": "0", "module": "C1"}, {"value": "2.67045090723494E-08", "module": "C2"}, {"value": "4.93456582041878E-09", "module": "C3"}, {"value": "0", "module": "C4"}, {"value": "-1.17723792420476E-06", "module": "D"}]}}, {"referenceToLCIAMethodDataSet": {"shortDescription": [{"value": "Acidification potential of land and water (AP)", "lang": "en"}, {"value": "Versauerungspotenzial von Boden und Wasser (AP)", "lang": "de"}], "type": "LCIA method data set", "refObjectId": "b5c611c6-def3-11e6-bf01-fe55135034f3", "uri": "../lciamethods/b5c611c6-def3-11e6-bf01-fe55135034f3.xml"}, "other": {"anies": [{"name": "referenceToUnitGroupDataSet", "value": {"shortDescription": [{"value": "mol H^(+) eq", "lang": "en"}], "type": "unit group data set", "refObjectId": "42e089ac-92bf-4bf2-8ca1-5fc40d18f2ed", "uri": "../unitgroups/42e089ac-92bf-4bf2-8ca1-5fc40d18f2ed.xml"}}, {"value": "0.0471782300560738", "module": "A1-A3"}, {"value": "0.00254991090856206", "module": "A4"}, {"value": "6.03726215801912E-05", "module": "A5"}, {"value": "0", "module": "C1"}, {"value": "0.000355777842507281", "module": "C2"}, {"value": "0.00052443092287442", "module": "C3"}, {"value": "0", "module": "C4"}, {"value": "-0.00913768722067594", "module": "D"}]}}, {"referenceToLCIAMethodDataSet": {"shortDescription": [{"value": "Eutrophication potential aquatic freshwater (EP-freshwater)", "lang": "en"}, {"value": "Eutrophierungspotenzial Süßwasser (EP-freshwater)", "lang": "de"}], "type": "LCIA method data set", "refObjectId": "b53ec18f-7377-4ad3-86eb-cc3f4f276b2b", "uri": "../lciamethods/b53ec18f-7377-4ad3-86eb-cc3f4f276b2b.xml"}, "other": {"anies": [{"name": "referenceToUnitGroupDataSet", "value": {"shortDescription": [{"value": "kg P eq", "lang": "en"}], "type": "unit group data set", "refObjectId": "0429039d-a61d-4590-ba67-aa4a20a810a1", "uri": "../unitgroups/0429039d-a61d-4590-ba67-aa4a20a810a1.xml"}}, {"value": "0.000286389584971746", "module": "A1-A3"}, {"value": "5.99402479949494E-06", "module": "A4"}, {"value": "2.55412541014921E-08", "module": "A5"}, {"value": "0", "module": "C1"}, {"value": "9.67071080506068E-07", "module": "C2"}, {"value": "1.01811895962747E-05", "module": "C3"}, {"value": "0", "module": "C4"}, {"value": "-0.000142840440949096", "module": "D"}]}}, {"referenceToLCIAMethodDataSet": {"shortDescription": [{"value": "Eutrophication potential aquatic marine (EP-marine)", "lang": "en"}, {"value": "Eutrophierungspotenzial Salzwasser (EP-marine)", "lang": "de"}], "type": "LCIA method data set", "refObjectId": "b5c619fa-def3-11e6-bf01-fe55135034f3", "uri": "../lciamethods/b5c619fa-def3-11e6-bf01-fe55135034f3.xml"}, "other": {"anies": [{"name": "referenceToUnitGroupDataSet", "value": {"shortDescription": [{"value": "kg N eq", "lang": "en"}], "type": "unit group data set", "refObjectId": "d05bb823-ecdf-4686-8c40-bf1d9257859f", "uri": "../unitgroups/d05bb823-ecdf-4686-8c40-bf1d9257859f.xml"}}, {"value": "0.00812125491886854", "module": "A1-A3"}, {"value": "0.000558641264918735", "module": "A4"}, {"value": "2.72334748494332E-05", "module": "A5"}, {"value": "0", "module": "C1"}, {"value": "7.45712935236321E-05", "module": "C2"}, {"value": "7.12065195333581E-05", "module": "C3"}, {"value": "0", "module": "C4"}, {"value": "-0.000958732581804838", "module": "D"}]}}, {"referenceToLCIAMethodDataSet": {"shortDescription": [{"value": "Eutrophication potential terrestrial (EP-terrestrial)", "lang": "en"}, {"value": "Eutrophierungspotenzial Land (EP-terrestrial)", "lang": "de"}], "type": "LCIA method data set", "refObjectId": "b5c614d2-def3-11e6-bf01-fe55135034f3", "uri": "../lciamethods/b5c614d2-def3-11e6-bf01-fe55135034f3.xml"}, "other": {"anies": [{"name": "referenceToUnitGroupDataSet", "value": {"shortDescription": [{"value": "mol N eq", "lang": "en"}], "type": "unit group data set", "refObjectId": "71b4d617-0ec9-4d3f-b65e-e438940c2401", "uri": "../unitgroups/71b4d617-0ec9-4d3f-b65e-e438940c2401.xml"}}, {"value": "0.109593327826439", "module": "A1-A3"}, {"value": "0.00621038954581186", "module": "A4"}, {"value": "0.000306623661036787", "module": "A5"}, {"value": "0", "module": "C1"}, {"value": "0.000831384626614957", "module": "C2"}, {"value": "0.000813859955770277", "module": "C3"}, {"value": "0", "module": "C4"}, {"value": "-0.0107608789873531", "module": "D"}]}}, {"referenceToLCIAMethodDataSet": {"shortDescription": [{"value": "Formation potential of tropospheric ozone photochemical oxidants (POCP)", "lang": "en"}, {"value": "Bildungspotential für troposphärisches Ozon (POCP)", "lang": "de"}], "type": "LCIA method data set", "refObjectId": "b5c610fe-def3-11e6-bf01-fe55135034f3", "uri": "../lciamethods/b5c610fe-def3-11e6-bf01-fe55135034f3.xml"}, "other": {"anies": [{"name": "referenceToUnitGroupDataSet", "value": {"shortDescription": [{"value": "kg NMVOC eq", "lang": "en"}], "type": "unit group data set", "refObjectId": "d27c25f8-fbc1-44c6-b47b-4adbae4199c6", "uri": "../unitgroups/d27c25f8-fbc1-44c6-b47b-4adbae4199c6.xml"}}, {"value": "0.0302246351260903", "module": "A1-A3"}, {"value": "0.00225281269666171", "module": "A4"}, {"value": "9.10355787499132E-05", "module": "A5"}, {"value": "0", "module": "C1"}, {"value": "0.000301774132641739", "module": "C2"}, {"value": "0.00022904388200886", "module": "C3"}, {"value": "0", "module": "C4"}, {"value": "-0.00471290031624789", "module": "D"}]}}, {"referenceToLCIAMethodDataSet": {"shortDescription": [{"value": "Abiotic depletion potential for non fossil resources (ADPE)", "lang": "en"}, {"value": "Potenzial für den abiotischen Abbau nicht fossiler Ressourcen (ADPE)", "lang": "de"}], "type": "LCIA method data set", "refObjectId": "b2ad6494-c78d-11e6-9d9d-cec0c932ce01", "uri": "../lciamethods/b2ad6494-c78d-11e6-9d9d-cec0c932ce01.xml"}, "other": {"anies": [{"name": "referenceToUnitGroupDataSet", "value": {"shortDescription": [{"value": "kg Sb eq", "lang": "en"}], "type": "unit group data set", "refObjectId": "54ccd2d9-a32a-4fc2-923d-f2c8c93e89d4", "uri": "../unitgroups/54ccd2d9-a32a-4fc2-923d-f2c8c93e89d4.xml"}}, {"value": "8.92522638177695E-05", "module": "A1-A3"}, {"value": "2.97913343174834E-06", "module": "A4"}, {"value": "7.3966904432095E-09", "module": "A5"}, {"value": "0", "module": "C1"}, {"value": "5.42125905685887E-07", "module": "C2"}, {"value": "2.70301311887349E-07", "module": "C3"}, {"value": "0", "module": "C4"}, {"value": "-3.27388764541467E-06", "module": "D"}]}}, {"referenceToLCIAMethodDataSet": {"shortDescription": [{"value": "Abiotic depletion potential for fossil resources (ADPF)", "lang": "en"}, {"value": "Potenzial für den abiotischen Abbau fossiler Brennstoffe (ADPF)", "lang": "de"}], "type": "LCIA method data set", "refObjectId": "b2ad6110-c78d-11e6-9d9d-cec0c932ce01", "uri": "../lciamethods/b2ad6110-c78d-11e6-9d9d-cec0c932ce01.xml"}, "other": {"anies": [{"name": "referenceToUnitGroupDataSet", "value": {"shortDescription": [{"value": "MJ", "lang": "en"}], "type": "unit group data set", "refObjectId": "93a60a57-a3c8-11da-a746-0800200c9a66", "uri": "../unitgroups/93a60a57-a3c8-11da-a746-0800200c9a66.xml"}}, {"value": "148.933200287231", "module": "A1-A3"}, {"value": "12.7720685441465", "module": "A4"}, {"value": "0.0672836785371035", "module": "A5"}, {"value": "0", "module": "C1"}, {"value": "1.77330647723327", "module": "C2"}, {"value": "2.04800352208267", "module": "C3"}, {"value": "0", "module": "C4"}, {"value": "-154.66792238605", "module": "D"}]}}, {"referenceToLCIAMethodDataSet": {"shortDescription": [{"value": "Water use (WDP)", "lang": "en"}, {"value": "Wassernutzung (WDP)", "lang": "de"}], "type": "LCIA method data set", "refObjectId": "b2ad66ce-c78d-11e6-9d9d-cec0c932ce01", "uri": "../lciamethods/b2ad66ce-c78d-11e6-9d9d-cec0c932ce01.xml"}, "other": {"anies": [{"name": "referenceToUnitGroupDataSet", "value": {"shortDescription": [{"value": "m^(3) world eq deprived", "lang": "en"}], "type": "unit group data set", "refObjectId": "6ae2df01-888e-46c8-b17d-49fa3869b476", "uri": "../unitgroups/6ae2df01-888e-46c8-b17d-49fa3869b476.xml"}}, {"value": "8.27149848457968", "module": "A1-A3"}, {"value": "0.0387804378799259", "module": "A4"}, {"value": "0.000357597634632564", "module": "A5"}, {"value": "0", "module": "C1"}, {"value": "0.00587974484283571", "module": "C2"}, {"value": "0.0237808889466005", "module": "C3"}, {"value": "0", "module": "C4"}, {"value": "-0.140547538077576", "module": "D"}]}}, {"referenceToLCIAMethodDataSet": {"shortDescription": [{"value": "Incidence of disease due to PM emissions (PM)", "lang": "en"}, {"value": "Auftreten von Krankheiten aufgrund von Feinstaubemissionen (PM)", "lang": "de"}], "type": "LCIA method data set", "refObjectId": "b5c602c6-def3-11e6-bf01-fe55135034f3", "uri": "../lciamethods/b5c602c6-def3-11e6-bf01-fe55135034f3.xml"}, "other": {"anies": [{"name": "referenceToUnitGroupDataSet", "value": {"shortDescription": [{"value": "Disease incidence", "lang": "en"}], "type": "unit group data set", "refObjectId": "3883559b-648f-4afc-8ba2-0bd24f3affa3", "uri": "../unitgroups/3883559b-648f-4afc-8ba2-0bd24f3affa3.xml"}}, {"value": "3.8177034031238E-07", "module": "A1-A3"}, {"value": "5.39981871510243E-08", "module": "A4"}, {"value": "8.48416206570756E-10", "module": "A5"}, {"value": "0", "module": "C1"}, {"value": "6.52237727919618E-09", "module": "C2"}, {"value": "1.5976460756463E-09", "module": "C3"}, {"value": "0", "module": "C4"}, {"value": "-7.12347599268411E-09", "module": "D"}]}}, {"referenceToLCIAMethodDataSet": {"shortDescription": [{"value": "Human exposure efficiency relative to U235 (IR)", "lang": "en"}, {"value": "Wirkung durch Exposition des Menschen mit U235 (IR)", "lang": "de"}], "type": "LCIA method data set", "refObjectId": "b5c632be-def3-11e6-bf01-fe55135034f3", "uri": "../lciamethods/b5c632be-def3-11e6-bf01-fe55135034f3.xml"}, "other": {"anies": [{"name": "referenceToUnitGroupDataSet", "value": {"shortDescription": [{"value": "kBq U235 eq", "lang": "en"}], "type": "unit group data set", "refObjectId": "456b05bf-1415-44a9-9993-02452f554c09", "uri": "../unitgroups/456b05bf-1415-44a9-9993-02452f554c09.xml"}}, {"value": "0.301967253909826", "module": "A1-A3"}, {"value": "0.0554516297658354", "module": "A4"}, {"value": "0.000267225429193828", "module": "A5"}, {"value": "0", "module": "C1"}, {"value": "0.00771194196285957", "module": "C2"}, {"value": "0.0181044644370452", "module": "C3"}, {"value": "0", "module": "C4"}, {"value": "-0.278897291509286", "module": "D"}]}}, {"referenceToLCIAMethodDataSet": {"shortDescription": [{"value": "Comparative toxic unit for ecosystems (ETP-fw)", "lang": "en"}, {"value": "Toxizitätsvergleichseinheit für Ökosysteme (ETP-fw)", "lang": "de"}], "type": "LCIA method data set", "refObjectId": "ee1082d1-b0f7-43ca-a1f0-21e2a4a74511", "uri": "../lciamethods/ee1082d1-b0f7-43ca-a1f0-21e2a4a74511.xml"}, "other": {"anies": [{"name": "referenceToUnitGroupDataSet", "value": {"shortDescription": [{"value": "CTUe", "lang": "en"}], "type": "unit group data set", "refObjectId": "aa959ded-f1eb-4efb-9c5c-2d60be36b3e6", "uri": "../unitgroups/aa959ded-f1eb-4efb-9c5c-2d60be36b3e6.xml"}}, {"value": "176.218549070189", "module": "A1-A3"}, {"value": "10.0161338060205", "module": "A4"}, {"value": "0.0554013776024547", "module": "A5"}, {"value": "0", "module": "C1"}, {"value": "1.44756065515412", "module": "C2"}, {"value": "1.16257851119687", "module": "C3"}, {"value": "0", "module": "C4"}, {"value": "-9.58334626438463", "module": "D"}]}}, {"referenceToLCIAMethodDataSet": {"shortDescription": [{"value": "Comparative toxic unit for humans (carcinogenic) (HTP-c)", "lang": "en"}, {"value": "Toxizitätsvergleichseinheit für Menschen (krebserregend) (HTP-c)", "lang": "de"}], "type": "LCIA method data set", "refObjectId": "2299222a-bbd8-474f-9d4f-4dd1f18aea7c", "uri": "../lciamethods/2299222a-bbd8-474f-9d4f-4dd1f18aea7c.xml"}, "other": {"anies": [{"name": "referenceToUnitGroupDataSet", "value": {"shortDescription": [{"value": "CTUh", "lang": "en"}], "type": "unit group data set", "refObjectId": "d4c9523e-2d7e-49fd-8469-998f547d3a70", "uri": "../unitgroups/d4c9523e-2d7e-49fd-8469-998f547d3a70.xml"}}, {"value": "4.98671567074505E-08", "module": "A1-A3"}, {"value": "3.22477527885658E-10", "module": "A4"}, {"value": "3.2801787341852E-11", "module": "A5"}, {"value": "0", "module": "C1"}, {"value": "5.23486764434746E-11", "module": "C2"}, {"value": "5.50812083566065E-11", "module": "C3"}, {"value": "0", "module": "C4"}, {"value": "1.27733510007222E-09", "module": "D"}]}}, {"referenceToLCIAMethodDataSet": {"shortDescription": [{"value": "Comparative toxic unit for humans (noncarcinogenic) (HTP-nc)", "lang": "en"}, {"value": "Toxizitätsvergleichseinheit für Menschen (nicht krebserregend) (HTP-nc)", "lang": "de"}], "type": "LCIA method data set", "refObjectId": "3af763a5-b7a1-48c9-9cee-1f223481fcef", "uri": "../lciamethods/3af763a5-b7a1-48c9-9cee-1f223481fcef.xml"}, "other": {"anies": [{"name": "referenceToUnitGroupDataSet", "value": {"shortDescription": [{"value": "CTUh", "lang": "en"}], "type": "unit group data set", "refObjectId": "d4c9523e-2d7e-49fd-8469-998f547d3a70", "uri": "../unitgroups/d4c9523e-2d7e-49fd-8469-998f547d3a70.xml"}}, {"value": "1.29708583338069E-07", "module": "A1-A3"}, {"value": "1.01789577655373E-08", "module": "A4"}, {"value": "1.21683844243152E-10", "module": "A5"}, {"value": "0", "module": "C1"}, {"value": "1.40993402734316E-09", "module": "C2"}, {"value": "9.9913202739551E-10", "module": "C3"}, {"value": "0", "module": "C4"}, {"value": "2.49990325321437E-09", "module": "D"}]}}, {"referenceToLCIAMethodDataSet": {"shortDescription": [{"value": "Soil quality index (SQP)", "lang": "en"}, {"value": "Bodenqualitätsindex (SQP)", "lang": "de"}], "type": "LCIA method data set", "refObjectId": "b2ad6890-c78d-11e6-9d9d-cec0c932ce01", "uri": "../lciamethods/b2ad6890-c78d-11e6-9d9d-cec0c932ce01.xml"}, "other": {"anies": [{"name": "referenceToUnitGroupDataSet", "value": {"shortDescription": [{"value": "SQP", "lang": "en"}], "type": "unit group data set", "refObjectId": "f130951c-e67f-4f7f-8dd4-665de3974e18", "uri": "../unitgroups/f130951c-e67f-4f7f-8dd4-665de3974e18.xml"}}, {"value": "378.492298402527", "module": "A1-A3"}, {"value": "8.88271783648281", "module": "A4"}, {"value": "0.0133803396353477", "module": "A5"}, {"value": "0", "module": "C1"}, {"value": "1.04847942863562", "module": "C2"}, {"value": "0.31558391496579", "module": "C3"}, {"value": "0", "module": "C4"}, {"value": "-4.04974809813168", "module": "D"}]}}]}, "otherAttributes": {"{http://www.indata.network/EPD/2019}epd-version": "1.2"}, "version": "1.1", "locations": "../ILCDLocations.xml"}