{"processInformation": {"dataSetInformation": {"UUID": "3a888531-f0de-4e0f-88c2-530bebdc7b8e", "name": {"baseName": [{"value": "Laminatboden", "lang": "de"}, {"value": "Laminate flooring", "lang": "en"}], "functionalUnitFlowProperties": [{"lang": "de"}]}, "classificationInformation": {"classification": [{"class": [{"value": "Holz", "level": 0, "classId": "3"}, {"value": "Holzböden", "level": 1, "classId": "3.3"}, {"value": "Laminat", "level": 2, "classId": "3.3.01"}], "name": "OEKOBAU.DAT"}, {"class": [{"value": "02 Bauprodukte", "level": 0}, {"value": "Bodenbeläge", "level": 1}, {"value": "Bodenbeläge", "level": 2}], "name": "IBUCategories"}]}, "generalComment": [{"value": "Parador Laminatbden zhlen zur Gruppe der Hartboden-Elemente und zeichnen sich durch eine hochabriebsfeste Deckschicht aus, die sich mithilfe einer patentierten Klick-Verbindung zur schwimmenden Verlegung eignen. Durch das bedruckte und imprgnierte Dekorpapier wird eine individuelle Optik erzielt. Ein spezielles Herstellungsverfahren erzeugt eine Oberflchenstruktur. Laminatbden sind in verschiedenen Dielenformaten erhltlich, die auf den Lngs- und Querseiten mit einer hochprzisen Klickverbindung versehen sind. Die fertigen Dielen werden im Werk zum Schutz vor Beschdigung in Kartons und in PE-Folie verpackt. Die jeweiligen Produktionsanteile aller im Werk Coesfeld hergestellten Laminatbden werden in die Berechnung der Durchschnittswerte einbezogen.", "lang": "de"}, {"value": "Parador laminate flooring is part of the group of hard flooring elements characterized by a highly abrasion-resistant top layer suitable for floating installation using a patented click connection. An individual look is achieved by the printed and impregnated decor paper. A special manufacturing process creates a texture on the surface. Laminate floorings are available in various plank formats, which are contoured on the long and short sides with a highly precise click connection. The finished planks are packed in boxes and in pe-foil at the factory to protect them from damage. The respective production shares of all laminate flooring produced at the Coesfeld plant is included in the calculation of averages.", "lang": "en"}]}, "quantitativeReference": {"referenceToReferenceFlow": [0]}, "time": {"referenceYear": 2024, "dataSetValidUntil": 2029, "other": {"anies": [{"name": "publicationDateOfEPD", "value": 1731369600000}]}}, "geography": {"locationOfOperationSupplyOrProduction": {"location": "DE"}}, "technology": {"technologyDescriptionAndIncludedProcesses": [{"value": "Illustration of the Direct Pressed Laminate flooring (DPL) manufacturing process: The overlay, decor paper, core board (HDF), and backing materials are thermally pressed together in one working step in a short-cycle press. Through an irreversible polycondensation reaction during compression, the impregnating resin (melamine-urea-formaldehyde) is three-dimensionally cross-linked under thermal input. The chemically stable binding agents are thus firmly bound in the wood. After pressing, the semi-finished formats acclimatise to ambient temperature. After an acclimatisation period, the semi-finished formats are cut according to the product formats and given a lengthways and crossways profile. After quality control of the individual laminate flooring elements, they are packed in half-shell cartons and shrink-wrapped. These individual packaging units are stacked on pallets according to the different formats. All processes are continually inspected and documented as part of the in-house Factory Production Control (FPC). \nTechnische Daten: \nStrukturelle Daten \nEs gelten die Leistungswerte des Produkts entsprechend der Leistungserklrung in Bezug auf dessen wesentliche Merkmale gem EN 13329:2017-12. \nDeklarierte Einheit: \nDie deklarierte Einheit ist 1 m2 des nach der Produktionsmenge gewichteten Durchschnitts der Laminat-Bodenbelge inklusive Verpackungsmaterialien.", "lang": "de"}, {"value": "Illustration of the Direct Pressed Laminate flooring (DPL) manufacturing process: The overlay, decor paper, core board (HDF), and backing materials are thermally pressed together in one production step in a short-cycle press. Through an irreversible polycondensation reaction during compression, the impregnating resin (melamine-urea-formaldehyde) is three-dimensionally cross- linked under thermal input. The chemically stable binding agents are thus firmly bound in the wood. After pressing, the semi-finished formats acclimatize to ambient temperature. After an acclimatization period, the semi-finished formats are cut according to the product formats and given a lengthways and crossways profile. After quality control of the individual laminate flooring elements, they are packed in half- shell cartons and shrink-wrapped. These individual packaging units are stacked on pallets according to the different formats. All processes are continually inspected and documented as part of the in-house Factory Production Control (FPC). \nTechnical data: \nStructural data \nThe performance values of the product according to the declaration of performance shall apply with regard to its essential characteristics according to EN 13329:2017-12. \nDeclared unit: \nThe declared unit is 1 m2 of the laminate flooring including packaging materials of the weighted average according to the production quantity.", "lang": "en"}], "technologicalApplicability": [{"value": "Laminatbden eignen sich sowohl fr die schwimmende Verlegung im Innenbereich von Neubauten als auch fr Sanierungen. Sie knnen sowohl auf Estrich als auch auf anderen mineralischen Unterbden, Holz, Fliesen oder PVC verlegt werden. Die Grundstze fachgerechter Verlegung knnen der beiliegenden Verlegeanleitung bzw. dem Ratgeber fr Laminatbden entnommen werden. \nZu finden unter: https://parador.de/services/downloads/laminat und dort unter der Rubrik \"Ratgeber\".", "lang": "de"}, {"value": "Laminate floorings are suitable for floating installation indoors in new buildings as well as for renovations. They can be installed on screed as well as other mineral subfloors, wood, tiles or PVC. The principles of proper installation can be found in the enclosed installation instructions or in the Guide for Laminate flooring. \nTo be found here: https://parador.de/en/services/downloads/laminate-flooring and there under the heading and there under the heading Guide.", "lang": "en"}]}}, "modellingAndValidation": {"LCIMethodAndAllocation": {"typeOfDataSet": "EPD", "referenceToLCAMethodDetails": [{"shortDescription": [{"value": "Bodenbeläge.pdf", "lang": "de"}], "type": "source data set", "refObjectId": "e6b9b35b-34b8-4934-ad67-41355e0c9b7c"}], "other": {"anies": [{"name": "subType", "value": "average dataset"}]}}, "dataSourcesTreatmentAndRepresentativeness": {"referenceToDataSource": [{"shortDescription": [{"value": "GaBi Database (all versions)", "lang": "de"}], "type": "source data set", "refObjectId": "28d74cc0-db8b-4d7e-bc44-5f6d56ce0c4a"}, {"shortDescription": [{"value": "Sphera MLC (fka GaBi) CUP 2023.02", "lang": "de"}], "type": "source data set", "refObjectId": "cb600d3b-e85a-42b3-b059-5591e2757fbb"}], "useAdviceForDataSet": [{"value": "Gültigkeitsbereich: \nDiese EPD gilt fr die Produktion von Laminatbden im deutschen Produktionswerk der Parador GmbH in Coesfeld. Bercksichtigt wurden dabei smtliche Produkttypen, die im Zeitraum 01.04.2022 – 31.03.2023 hergestellt wurden. \nSystemgrenze: \nTyp der EPD: Wiege bis Werkstor mit Optionen, Module C1–C4 und Modul D und Zusatzmodule (A4–A5 und B2–B3). \n\nModule A1–A3 \nIn der Produktionsphase, die Beschaffung der Rohstoffe inklusive der dazugehrigen Vorketten, die notwendigen Transporte zum Werk sowie der Energieaufwand zur Herstellung der Laminatbodenbelge. Zur Modellierung der Rohstoffgewinnung bis hin zur Herstellung der Vorprodukte (A1) werden generische Datenstze verwendet, um die Systemgrenzen (Cradle to Gate) fr die Einsatzstoffe zu modellieren. Der Transport (A2) zum Werk wird durch generische Datenstze abgedeckt. Die Fertigungsphase (A3), die insbesondere die Extrusion umfasst, ist mit herstellerspezifischen Material- und Energiedaten abgebildet, wobei die vorgelagerten Phasen wiederum anhand generischer Datenstze dargestellt sind. Die Produktionsabflle werden bis zur vollstndigen Aufbereitung bzw. bis zum Erreichen des End-of-Waste-Status (EoW) erfasst. \n\nModul A4 \nIn Modul A4 werden die Transporte zur Baustelle auf Basis der durchschnittlichen Entfernungen zu den Kunden analysiert. \n\nModul A5 \nIn Modul A5 werden die Verpackungen, die beim Einbau des Bauteils auf der Baustelle anfallen, energetisch (Polyethylenfolie) oder stofflich (Kartonagen) verwertet. Die Transportaufwendungen zur Entsorgung werden ebenfalls in Modul A5 bercksichtigt, die Gutschriften und Lasten in Modul D. Die sich aus dem Kartonrecycling ergebenden Gutschriften wurden aufgrund fehlender Daten herausgerechnet. \n\nModul B2 \nModul B2 umfasst die Reinigung des Laminatbodens inklusive der bentigten Hilfsmittel sowie die Behandlung von Abfllen und Abwasser. \n\nModul B3 \nModul B3 befasst sich mit der Reparatur des Laminatbodens einschlielich der Behandlung der dabei anfallenden Abflle. \n\nModul C1 \nModul C1 beschreibt die Aufwendungen nach dem Produktlebensende fr die Demontage oder Rckbau des Produkts aus dem Gebude. In diesem Fall kann davon ausgegangen werden, dass der Rckbau manuell erfolgt. \n\nModul C2 \nIn Modul C2 werden die Transporte zu den Entsorgungsprozessen betrachtet. \n\nModul C3 \nModul C3 beinhaltet die notwendigen Prozesse fr die Abfallbehandlung am Ende des Produktlebenswegs. Betrachtet wird hier eine Bauschuttaufbereitungsanlage. \n\nModul C4 \nModul C4 beschreibt die Deponierung des Produktes am Ende des Lebenswegs.", "lang": "de"}, {"value": "Scope: \nThis EPD applies to the production of laminate flooring in the German production plant of Parador GmbH in Coesfeld. All product types manufactured in the period 01.04.2022 - 31.03.2023 were taken into account. \nSystem boundary: \nType of EPD:\nFrom the cradle to the factory gate with options, modules C1-C4 and module D and additional modules (A4-A5 and B2-B3). \n\nModules A1-A3 \nAt the production stage, the procurement of raw materials including the corresponding upstream chains, the necessary transport to the plant and the energy required for the production of the the energy required to produce the laminat floor coverings. To model the extraction of raw materials up to the production of the preliminary products (A1), generic generic data sets are used to model the system boundaries system boundaries (cradle to gate) for the input materials. Transport (A2) to the plant is covered by generic data records. are covered. The manufacturing phase (A3), which includes extrusion in particular, is mapped with manufacturer-specific material and energy mapped with manufacturer-specific material and energy data, whereby the upstream are again mapped using generic data sets. The production waste is mapped until it is completely treatment or until the end-of-waste status (EoW) is reached. \n\nModule A4 \nIn Module A4, transport to the construction site is analysed on the basis of the average distances to the customers.\n\nModule A5\nIn Module A5, the packaging that is generated during of the assembly component on the construction site are utilised for energy (polyethylene film) or recycling (cardboard packaging). The transport costs for disposal are also taken into account in module A5, the benefits and burdens in module D.\nThe resulting benefits from cardboard recycling were cut off due to a lack of data.\n\nModule B2 \nModule B2 covers the cleaning of the laminate flooring, including the necessary auxiliary materials as well as the treatment of the waste and wastewater. \n\nModule B3 \nModule B3 deals with the repair of the laminate flooring including the treatment of the resulting waste.\n\nModule C1\nModule C1 describes the expenses after end of product life for dismantling or demolishing the product from the building. In this case, it can be assumed that that the dismantling is carried out manually. No processes are therefore considered/modelled in module C1.\n\nModule C2 \nIn Module C2, the transports to the disposal processes are considered.\n\nModule C3 \nModule C3 covers the necessary processes for waste treatment at the end of the product life cycle. A construction waste processing plant is considered here.\n\nModule C4 \nModule C4 describes the landfilling of the product at the end of the life cycle.", "lang": "en"}], "other": {"anies": [{"name": "referenceToOriginalEPD", "value": {"shortDescription": {"value": "Laminatboden.pdf", "defaultValue": "Laminatboden.pdf", "lstrings": [{"lang": "de", "value": "Laminatboden.pdf"}]}, "type": "source data set", "uuid": {"uuid": "de57737d-c7ea-4b17-a960-19b1e2403704"}, "refObjectId": "de57737d-c7ea-4b17-a960-19b1e2403704", "resourceURLs": ["https://oekobaudat.de/OEKOBAU.DAT/resource/sources/de57737d-c7ea-4b17-a960-19b1e2403704/Laminatboden_22908.pdf?version=00.01.000"]}}]}}, "validation": {"review": [{"referenceToNameOfReviewerAndInstitution": [{"shortDescription": [{"value": "Institut Bauen und Umwelt e. V.", "lang": "de"}], "type": "contact data set", "refObjectId": "d111dbec-b024-4be5-86c5-752d6eb2cf95", "uri": "../contacts/d111dbec-b024-4be5-86c5-752d6eb2cf95.xml"}], "type": "Accredited third party review"}]}, "complianceDeclarations": {"compliance": [{"referenceToComplianceSystem": {"shortDescription": [{"value": "DIN EN 15804+A2", "lang": "de"}], "type": "source data set", "refObjectId": "c0016b33-8cf7-415c-ac6e-deba0d21440d", "uri": "../sources/c0016b33-8cf7-415c-ac6e-deba0d21440d.xml"}}, {"referenceToComplianceSystem": {"shortDescription": [{"value": "ISO 14025", "lang": "de"}], "type": "source data set", "refObjectId": "4f2eb655-6e44-4874-a95a-e28f5442cd4d", "uri": "../sources/4f2eb655-6e44-4874-a95a-e28f5442cd4d.xml"}}]}}, "administrativeInformation": {"commissionerAndGoal": {"referenceToCommissioner": [{"shortDescription": [{"value": "Parador GmbH", "lang": "de"}], "type": "contact data set", "refObjectId": "0861a318-be95-448b-b08e-751d226e2c2c", "uri": "../contacts/0861a318-be95-448b-b08e-751d226e2c2c.xml"}]}, "dataGenerator": {"referenceToPersonOrEntityGeneratingTheDataSet": [{"shortDescription": [{"value": "brands and values GmbH", "lang": "de"}], "type": "contact data set", "refObjectId": "6b539b8a-10e3-4004-8ccc-a79f169aa339", "uri": "../contacts/6b539b8a-10e3-4004-8ccc-a79f169aa339.xml"}]}, "dataEntryBy": {"timeStamp": 1731369600000, "referenceToDataSetFormat": [{"shortDescription": [{"value": "ILCD Format", "lang": "de"}], "type": "source data set", "refObjectId": "a97a0155-0234-4b87-b4ce-a45da52f2a40", "uri": "../sources/a97a0155-0234-4b87-b4ce-a45da52f2a40.xml"}, {"shortDescription": [{"value": "EPD-Datenformaterweiterungen v1.2", "lang": "de"}, {"value": "EPD Data Format Extensions v1.2", "lang": "en"}], "type": "source data set", "refObjectId": "a29449fd-aa2f-4de8-b5d7-4b06b43c6fde", "uri": "../sources/a29449fd-aa2f-4de8-b5d7-4b06b43c6fde.xml"}]}, "publicationAndOwnership": {"dataSetVersion": "00.02.000", "referenceToRegistrationAuthority": {"shortDescription": [{"value": "Institut Bauen und Umwelt e. V.", "lang": "de"}], "type": "contact data set", "refObjectId": "d111dbec-b024-4be5-86c5-752d6eb2cf95", "uri": "../contacts/d111dbec-b024-4be5-86c5-752d6eb2cf95.xml"}, "registrationNumber": "EPD-PAR-20240253-IBC2-DE", "referenceToOwnershipOfDataSet": {"shortDescription": [{"value": "Parador GmbH", "lang": "de"}], "type": "contact data set", "refObjectId": "0861a318-be95-448b-b08e-751d226e2c2c", "uri": "../contacts/0861a318-be95-448b-b08e-751d226e2c2c.xml"}, "copyright": true, "licenseType": "Free of charge for all users and uses", "accessRestrictions": [{"value": "None", "lang": "en"}], "other": {"anies": [{"name": "referenceToPublisher", "value": {"shortDescription": [{"value": "Institut Bauen und Umwelt e. V.", "lang": "de"}], "type": "contact data set", "refObjectId": "d111dbec-b024-4be5-86c5-752d6eb2cf95", "uri": "../contacts/d111dbec-b024-4be5-86c5-752d6eb2cf95.xml"}}]}}}, "exchanges": {"exchange": [{"dataSetInternalID": 0, "referenceToFlowDataSet": {"shortDescription": [{"value": "Laminatboden (laminate flooring)", "lang": "de"}], "type": "flow data set", "refObjectId": "82f2aa53-98d7-94c3-37fd-995bfb8c1d7d", "uri": "../flows/82f2aa53-98d7-94c3-37fd-995bfb8c1d7d.xml"}, "meanAmount": 1.0, "referencesToDataSource": {}, "referenceFlow": true, "resolvedFlowVersion": "00.02.000", "resultingflowAmount": 1.0, "flowProperties": [{"name": [{"lang": "de", "value": "Fläche"}, {"lang": "en", "value": "Area"}], "uuid": "93a60a56-a3c8-19da-a746-0800200c9a66", "referenceFlowProperty": true, "meanValue": 1.0, "referenceUnit": "qm", "unitGroupUUID": "c20a03d7-bd90-4569-bc94-66cfd364dfc8"}], "materialProperties": [{"name": "layer thickness", "value": "0.008", "unit": "m", "unitDescription": "meters"}, {"name": "grammage", "value": "7.46", "unit": "kg/m^2", "unitDescription": "kilograms per square meter"}], "typeOfFlow": "Product flow", "classification": {"classHierarchy": "Holz / Holzböden / Laminat", "name": "OEKOBAU.DAT"}}, {"dataSetInternalID": 1, "referenceToFlowDataSet": {"shortDescription": [{"value": "Erneuerbare Primärenergie als Energieträger (PERE)", "lang": "de"}, {"value": "Renewable primary energy as energy carrier (PERE)", "lang": "en"}], "type": "flow data set", "refObjectId": "20f32be5-0398-4288-9b6d-accddd195317", "uri": "../flows/20f32be5-0398-4288-9b6d-accddd195317.xml"}, "exchange direction": "INPUT", "other": {"anies": [{"name": "referenceToUnitGroupDataSet", "value": {"shortDescription": [{"value": "MJ", "lang": "de"}], "type": "unit group data set", "refObjectId": "93a60a57-a3c8-11da-a746-0800200c9a66", "uri": "../unitgroups/93a60a57-a3c8-11da-a746-0800200c9a66.xml"}}, {"value": "53.5696262452671", "module": "A1-A3"}, {"value": "0.0699441923232262", "module": "A4"}, {"value": "3.20754253253097", "module": "A5"}, {"value": "0.0059931483140337", "module": "B2"}, {"value": "0.000904873041745282", "module": "B3"}, {"value": "0", "module": "C1"}, {"value": "0.0477491834484014", "module": "C2"}, {"value": "118.47822710868", "module": "C3"}, {"value": "0", "module": "C4"}, {"value": "-15.8608748259108", "module": "D"}]}, "resolvedFlowVersion": "38.00.000", "flowProperties": [], "typeOfFlow": "Other flow", "classification": {"classHierarchy": "Quantities", "name": "GaBiCategories"}}, {"dataSetInternalID": 2, "referenceToFlowDataSet": {"shortDescription": [{"value": "Erneuerbare Primärenergie zur stofflichen Nutzung (PERM)", "lang": "de"}, {"value": "Renewable primary energy resources as material utilization (PERM)", "lang": "en"}], "type": "flow data set", "refObjectId": "fb3ec0de-548d-4508-aea5-00b73bf6f702", "uri": "../flows/fb3ec0de-548d-4508-aea5-00b73bf6f702.xml"}, "exchange direction": "INPUT", "other": {"anies": [{"name": "referenceToUnitGroupDataSet", "value": {"shortDescription": [{"value": "MJ", "lang": "de"}], "type": "unit group data set", "refObjectId": "93a60a57-a3c8-11da-a746-0800200c9a66", "uri": "../unitgroups/93a60a57-a3c8-11da-a746-0800200c9a66.xml"}}, {"value": "120.913", "module": "A1-A3"}, {"value": "0", "module": "A4"}, {"value": "-3.205", "module": "A5"}, {"value": "0", "module": "B2"}, {"value": "0", "module": "B3"}, {"value": "0", "module": "C1"}, {"value": "0", "module": "C2"}, {"value": "-117.708", "module": "C3"}, {"value": "0", "module": "C4"}, {"value": "0", "module": "D"}]}, "resolvedFlowVersion": "38.00.000", "flowProperties": [], "typeOfFlow": "Other flow", "classification": {"classHierarchy": "Quantities", "name": "GaBiCategories"}}, {"dataSetInternalID": 3, "referenceToFlowDataSet": {"shortDescription": [{"value": "Total erneuerbare Primärenergie (PERT)", "lang": "de"}, {"value": "Total use of renewable primary energy resources (PERT)", "lang": "en"}], "type": "flow data set", "refObjectId": "53f97275-fa8a-4cdd-9024-65936002acd0", "uri": "../flows/53f97275-fa8a-4cdd-9024-65936002acd0.xml"}, "exchange direction": "INPUT", "other": {"anies": [{"name": "referenceToUnitGroupDataSet", "value": {"shortDescription": [{"value": "MJ", "lang": "de"}], "type": "unit group data set", "refObjectId": "93a60a57-a3c8-11da-a746-0800200c9a66", "uri": "../unitgroups/93a60a57-a3c8-11da-a746-0800200c9a66.xml"}}, {"value": "174.482626245267", "module": "A1-A3"}, {"value": "0.0699441923232262", "module": "A4"}, {"value": "0.00254253253097306", "module": "A5"}, {"value": "0.0059931483140337", "module": "B2"}, {"value": "0.000904873041745282", "module": "B3"}, {"value": "0", "module": "C1"}, {"value": "0.0477491834484014", "module": "C2"}, {"value": "0.770227108679687", "module": "C3"}, {"value": "0", "module": "C4"}, {"value": "-15.8608748259108", "module": "D"}]}, "resolvedFlowVersion": "38.00.000", "flowProperties": [], "typeOfFlow": "Other flow", "classification": {"classHierarchy": "Quantities / Environmental quantities / EPD EN 15804 / LCI indicators", "name": "GaBiCategories"}}, {"dataSetInternalID": 4, "referenceToFlowDataSet": {"shortDescription": [{"value": "Nicht-erneuerbare Primärenergie als Energieträger (PENRE)", "lang": "de"}, {"value": "Non renewable primary energy as energy carrier (PENRE)", "lang": "en"}], "type": "flow data set", "refObjectId": "ac857178-2b45-46ec-892a-a9a4332f0372", "uri": "../flows/ac857178-2b45-46ec-892a-a9a4332f0372.xml"}, "exchange direction": "INPUT", "other": {"anies": [{"name": "referenceToUnitGroupDataSet", "value": {"shortDescription": [{"value": "MJ", "lang": "de"}], "type": "unit group data set", "refObjectId": "93a60a57-a3c8-11da-a746-0800200c9a66", "uri": "../unitgroups/93a60a57-a3c8-11da-a746-0800200c9a66.xml"}}, {"value": "120.597987676979", "module": "A1-A3"}, {"value": "2.66196278325873", "module": "A4"}, {"value": "0.254469343437955", "module": "A5"}, {"value": "0.0100284566481485", "module": "B2"}, {"value": "0.0104780552158851", "module": "B3"}, {"value": "0", "module": "C1"}, {"value": "0.65860695785834", "module": "C2"}, {"value": "3.7319234896569", "module": "C3"}, {"value": "0", "module": "C4"}, {"value": "-54.149357515145", "module": "D"}]}, "resolvedFlowVersion": "38.00.000", "flowProperties": [], "typeOfFlow": "Other flow", "classification": {"classHierarchy": "Quantities", "name": "GaBiCategories"}}, {"dataSetInternalID": 5, "referenceToFlowDataSet": {"shortDescription": [{"value": "Nicht-erneuerbare Primärenergie zur stofflichen Nutzung (PENRM)", "lang": "de"}, {"value": "Non renewable primary energy as material utilization (PENRM)", "lang": "en"}], "type": "flow data set", "refObjectId": "1421caa0-679d-4bf4-b282-0eb850ccae27", "uri": "../flows/1421caa0-679d-4bf4-b282-0eb850ccae27.xml"}, "exchange direction": "INPUT", "other": {"anies": [{"name": "referenceToUnitGroupDataSet", "value": {"shortDescription": [{"value": "MJ", "lang": "de"}], "type": "unit group data set", "refObjectId": "93a60a57-a3c8-11da-a746-0800200c9a66", "uri": "../unitgroups/93a60a57-a3c8-11da-a746-0800200c9a66.xml"}}, {"value": "0.294", "module": "A1-A3"}, {"value": "0", "module": "A4"}, {"value": "-0.235", "module": "A5"}, {"value": "0", "module": "B2"}, {"value": "0", "module": "B3"}, {"value": "0", "module": "C1"}, {"value": "0", "module": "C2"}, {"value": "-0.059", "module": "C3"}, {"value": "0", "module": "C4"}, {"value": "0", "module": "D"}]}, "resolvedFlowVersion": "38.00.000", "flowProperties": [], "typeOfFlow": "Other flow", "classification": {"classHierarchy": "Quantities", "name": "GaBiCategories"}}, {"dataSetInternalID": 6, "referenceToFlowDataSet": {"shortDescription": [{"value": "Total nicht erneuerbare Primärenergie (PENRT)", "lang": "de"}, {"value": "Total use of non renewable primary energy resources (PENRT)", "lang": "en"}], "type": "flow data set", "refObjectId": "06159210-646b-4c8d-8583-da9b3b95a6c1", "uri": "../flows/06159210-646b-4c8d-8583-da9b3b95a6c1.xml"}, "exchange direction": "INPUT", "other": {"anies": [{"name": "referenceToUnitGroupDataSet", "value": {"shortDescription": [{"value": "MJ", "lang": "de"}], "type": "unit group data set", "refObjectId": "93a60a57-a3c8-11da-a746-0800200c9a66", "uri": "../unitgroups/93a60a57-a3c8-11da-a746-0800200c9a66.xml"}}, {"value": "120.891987676979", "module": "A1-A3"}, {"value": "2.66196278325873", "module": "A4"}, {"value": "0.0194693434379548", "module": "A5"}, {"value": "0.0100284566481485", "module": "B2"}, {"value": "0.0104780552158851", "module": "B3"}, {"value": "0", "module": "C1"}, {"value": "0.65860695785834", "module": "C2"}, {"value": "3.6729234896569", "module": "C3"}, {"value": "0", "module": "C4"}, {"value": "-54.149357515145", "module": "D"}]}, "resolvedFlowVersion": "38.00.000", "flowProperties": [], "typeOfFlow": "Other flow", "classification": {"classHierarchy": "Quantities / Environmental quantities / EPD EN 15804 / LCI indicators", "name": "GaBiCategories"}}, {"dataSetInternalID": 7, "referenceToFlowDataSet": {"shortDescription": [{"value": "Einsatz von Sekundärstoffen (SM)", "lang": "de"}, {"value": "Use of secondary material (SM)", "lang": "en"}], "type": "flow data set", "refObjectId": "c6a1f35f-2d09-4f54-8dfb-97e502e1ce92", "uri": "../flows/c6a1f35f-2d09-4f54-8dfb-97e502e1ce92.xml"}, "exchange direction": "INPUT", "other": {"anies": [{"name": "referenceToUnitGroupDataSet", "value": {"shortDescription": [{"value": "kg", "lang": "de"}], "type": "unit group data set", "refObjectId": "ad38d542-3fe9-439d-9b95-2f5f7752acaf", "uri": "../unitgroups/ad38d542-3fe9-439d-9b95-2f5f7752acaf.xml"}}, {"value": "0", "module": "A1-A3"}, {"value": "0", "module": "A4"}, {"value": "0", "module": "A5"}, {"value": "0", "module": "B2"}, {"value": "0", "module": "B3"}, {"value": "0", "module": "C1"}, {"value": "0", "module": "C2"}, {"value": "0", "module": "C3"}, {"value": "0", "module": "C4"}, {"value": "0.0131220608673099", "module": "D"}]}, "resolvedFlowVersion": "38.00.000", "flowProperties": [], "typeOfFlow": "Other flow", "classification": {"classHierarchy": "Quantities / Environmental quantities / EPD EN 15804 / LCI indicators", "name": "GaBiCategories"}}, {"dataSetInternalID": 8, "referenceToFlowDataSet": {"shortDescription": [{"value": "Erneuerbare Sekundärbrennstoffe (RSF)", "lang": "de"}, {"value": "Use of renewable secondary fuels (RSF)", "lang": "en"}], "type": "flow data set", "refObjectId": "64333088-a55f-4aa2-9a31-c10b07816787", "uri": "../flows/64333088-a55f-4aa2-9a31-c10b07816787.xml"}, "exchange direction": "INPUT", "other": {"anies": [{"name": "referenceToUnitGroupDataSet", "value": {"shortDescription": [{"value": "MJ", "lang": "de"}], "type": "unit group data set", "refObjectId": "93a60a57-a3c8-11da-a746-0800200c9a66", "uri": "../unitgroups/93a60a57-a3c8-11da-a746-0800200c9a66.xml"}}, {"value": "0", "module": "A1-A3"}, {"value": "0", "module": "A4"}, {"value": "0", "module": "A5"}, {"value": "0", "module": "B2"}, {"value": "0", "module": "B3"}, {"value": "0", "module": "C1"}, {"value": "0", "module": "C2"}, {"value": "0", "module": "C3"}, {"value": "0", "module": "C4"}, {"value": "0", "module": "D"}]}, "resolvedFlowVersion": "38.00.000", "flowProperties": [], "typeOfFlow": "Other flow", "classification": {"classHierarchy": "Quantities / Environmental quantities / EPD EN 15804 / LCI indicators", "name": "GaBiCategories"}}, {"dataSetInternalID": 9, "referenceToFlowDataSet": {"shortDescription": [{"value": "Nicht erneuerbare Sekundärbrennstoffe (NRSF)", "lang": "de"}, {"value": "Use of non renewable secondary fuels (NRSF)", "lang": "en"}], "type": "flow data set", "refObjectId": "89def144-d39a-4287-b86f-efde453ddcb2", "uri": "../flows/89def144-d39a-4287-b86f-efde453ddcb2.xml"}, "exchange direction": "INPUT", "other": {"anies": [{"name": "referenceToUnitGroupDataSet", "value": {"shortDescription": [{"value": "MJ", "lang": "de"}], "type": "unit group data set", "refObjectId": "93a60a57-a3c8-11da-a746-0800200c9a66", "uri": "../unitgroups/93a60a57-a3c8-11da-a746-0800200c9a66.xml"}}, {"value": "0", "module": "A1-A3"}, {"value": "0", "module": "A4"}, {"value": "0", "module": "A5"}, {"value": "0", "module": "B2"}, {"value": "0", "module": "B3"}, {"value": "0", "module": "C1"}, {"value": "0", "module": "C2"}, {"value": "0", "module": "C3"}, {"value": "0", "module": "C4"}, {"value": "0", "module": "D"}]}, "resolvedFlowVersion": "38.00.000", "flowProperties": [], "typeOfFlow": "Other flow", "classification": {"classHierarchy": "Quantities / Environmental quantities / EPD EN 15804 / LCI indicators", "name": "GaBiCategories"}}, {"dataSetInternalID": 10, "referenceToFlowDataSet": {"shortDescription": [{"value": "Einsatz von Süßwasserressourcen (FW)", "lang": "de"}, {"value": "Use of net fresh water (FW)", "lang": "en"}], "type": "flow data set", "refObjectId": "3cf952c8-f3a4-461d-8c96-96456ca62246", "uri": "../flows/3cf952c8-f3a4-461d-8c96-96456ca62246.xml"}, "exchange direction": "INPUT", "other": {"anies": [{"name": "referenceToUnitGroupDataSet", "value": {"shortDescription": [{"value": "m^3", "lang": "de"}], "type": "unit group data set", "refObjectId": "cd950537-0a98-4044-9ba7-9f9a68d0a504", "uri": "../unitgroups/cd950537-0a98-4044-9ba7-9f9a68d0a504.xml"}}, {"value": "0.031434371338528", "module": "A1-A3"}, {"value": "7.83696733956574E-05", "module": "A4"}, {"value": "0.000113783968553216", "module": "A5"}, {"value": "4.83920153800998E-06", "module": "B2"}, {"value": "1.84886069056493E-06", "module": "B3"}, {"value": "0", "module": "C1"}, {"value": "5.22982251004145E-05", "module": "C2"}, {"value": "0.0296926222807734", "module": "C3"}, {"value": "0", "module": "C4"}, {"value": "-0.0128501775619002", "module": "D"}]}, "resolvedFlowVersion": "38.00.000", "flowProperties": [], "typeOfFlow": "Other flow", "classification": {"classHierarchy": "Quantities / Environmental quantities / EPD EN 15804 / LCI indicators", "name": "GaBiCategories"}}, {"dataSetInternalID": 11, "referenceToFlowDataSet": {"shortDescription": [{"value": "Gefährlicher Abfall zur Deponie (HWD)", "lang": "de"}, {"value": "Hazardous waste disposed (HWD)", "lang": "en"}], "type": "flow data set", "refObjectId": "430f9e0f-59b2-46a0-8e0d-55e0e84948fc", "uri": "../flows/430f9e0f-59b2-46a0-8e0d-55e0e84948fc.xml"}, "exchange direction": "OUTPUT", "other": {"anies": [{"name": "referenceToUnitGroupDataSet", "value": {"shortDescription": [{"value": "kg", "lang": "de"}], "type": "unit group data set", "refObjectId": "ad38d542-3fe9-439d-9b95-2f5f7752acaf", "uri": "../unitgroups/ad38d542-3fe9-439d-9b95-2f5f7752acaf.xml"}}, {"value": "7.57823865196522E-08", "module": "A1-A3"}, {"value": "8.33872739229244E-12", "module": "A4"}, {"value": "1.8067729838782E-13", "module": "A5"}, {"value": "-7.84629995264113E-13", "module": "B2"}, {"value": "6.82343793811461E-13", "module": "B3"}, {"value": "0", "module": "C1"}, {"value": "2.0392561509215E-12", "module": "C2"}, {"value": "2.43476161291552E-10", "module": "C3"}, {"value": "0", "module": "C4"}, {"value": "-2.8364851337775E-09", "module": "D"}]}, "resolvedFlowVersion": "38.00.000", "flowProperties": [], "typeOfFlow": "Other flow", "classification": {"classHierarchy": "Quantities / Environmental quantities / EPD EN 15804 / LCI indicators", "name": "GaBiCategories"}}, {"dataSetInternalID": 12, "referenceToFlowDataSet": {"shortDescription": [{"value": "Entsorgter nicht gefährlicher Abfall (NHWD)", "lang": "de"}, {"value": "Non hazardous waste disposed (NHWD)", "lang": "en"}], "type": "flow data set", "refObjectId": "b29ef66b-e286-4afa-949f-62f1a7b4d7fa", "uri": "../flows/b29ef66b-e286-4afa-949f-62f1a7b4d7fa.xml"}, "exchange direction": "OUTPUT", "other": {"anies": [{"name": "referenceToUnitGroupDataSet", "value": {"shortDescription": [{"value": "kg", "lang": "de"}], "type": "unit group data set", "refObjectId": "ad38d542-3fe9-439d-9b95-2f5f7752acaf", "uri": "../unitgroups/ad38d542-3fe9-439d-9b95-2f5f7752acaf.xml"}}, {"value": "0.110878136216034", "module": "A1-A3"}, {"value": "0.000295595884818125", "module": "A4"}, {"value": "0.00020895417924947", "module": "A5"}, {"value": "7.47511048274456E-06", "module": "B2"}, {"value": "2.40077119986006E-05", "module": "B3"}, {"value": "0", "module": "C1"}, {"value": "0.000100397483676347", "module": "C2"}, {"value": "0.0919895782698659", "module": "C3"}, {"value": "0", "module": "C4"}, {"value": "-0.0268216824147373", "module": "D"}]}, "resolvedFlowVersion": "38.00.000", "flowProperties": [], "typeOfFlow": "Other flow", "classification": {"classHierarchy": "Quantities / Environmental quantities / EPD EN 15804 / LCI indicators", "name": "GaBiCategories"}}, {"dataSetInternalID": 13, "referenceToFlowDataSet": {"shortDescription": [{"value": "Entsorgter radioaktiver Abfall (RWD)", "lang": "de"}, {"value": "Radioactive waste disposed (RWD)", "lang": "en"}], "type": "flow data set", "refObjectId": "3449546e-52ad-4b39-b809-9fb77cea8ff6", "uri": "../flows/3449546e-52ad-4b39-b809-9fb77cea8ff6.xml"}, "exchange direction": "OUTPUT", "other": {"anies": [{"name": "referenceToUnitGroupDataSet", "value": {"shortDescription": [{"value": "kg", "lang": "de"}], "type": "unit group data set", "refObjectId": "ad38d542-3fe9-439d-9b95-2f5f7752acaf", "uri": "../unitgroups/ad38d542-3fe9-439d-9b95-2f5f7752acaf.xml"}}, {"value": "0.00459131507178836", "module": "A1-A3"}, {"value": "3.72443684354555E-06", "module": "A4"}, {"value": "3.98390210779603E-07", "module": "A5"}, {"value": "1.59406241972667E-06", "module": "B2"}, {"value": "8.41420486973071E-08", "module": "B3"}, {"value": "0", "module": "C1"}, {"value": "1.23254374881646E-06", "module": "C2"}, {"value": "0.000173355219540191", "module": "C3"}, {"value": "0", "module": "C4"}, {"value": "-0.00420894091701669", "module": "D"}]}, "resolvedFlowVersion": "38.00.000", "flowProperties": [], "typeOfFlow": "Other flow", "classification": {"classHierarchy": "Quantities / Environmental quantities / EPD EN 15804 / LCI indicators", "name": "GaBiCategories"}}, {"dataSetInternalID": 14, "referenceToFlowDataSet": {"shortDescription": [{"value": "Komponenten für die Wiederverwendung (CRU)", "lang": "de"}, {"value": "Components for re-use (CRU)", "lang": "en"}], "type": "flow data set", "refObjectId": "a2b32f97-3fc7-4af2-b209-525bc6426f33", "uri": "../flows/a2b32f97-3fc7-4af2-b209-525bc6426f33.xml"}, "exchange direction": "OUTPUT", "other": {"anies": [{"name": "referenceToUnitGroupDataSet", "value": {"shortDescription": [{"value": "kg", "lang": "de"}], "type": "unit group data set", "refObjectId": "ad38d542-3fe9-439d-9b95-2f5f7752acaf", "uri": "../unitgroups/ad38d542-3fe9-439d-9b95-2f5f7752acaf.xml"}}, {"value": "0", "module": "A1-A3"}, {"value": "0", "module": "A4"}, {"value": "0", "module": "A5"}, {"value": "0", "module": "B2"}, {"value": "0", "module": "B3"}, {"value": "0", "module": "C1"}, {"value": "0", "module": "C2"}, {"value": "0", "module": "C3"}, {"value": "0", "module": "C4"}, {"value": "0", "module": "D"}]}, "resolvedFlowVersion": "38.00.000", "flowProperties": [], "typeOfFlow": "Other flow", "classification": {"classHierarchy": "Quantities / Environmental quantities / EPD EN 15804 / LCI indicators", "name": "GaBiCategories"}}, {"dataSetInternalID": 15, "referenceToFlowDataSet": {"shortDescription": [{"value": "Stoffe zum Recycling (MFR)", "lang": "de"}, {"value": "Materials for recycling (MFR)", "lang": "en"}], "type": "flow data set", "refObjectId": "d7fe48a5-4103-49c8-9aae-b0b5dfdbd6ae", "uri": "../flows/d7fe48a5-4103-49c8-9aae-b0b5dfdbd6ae.xml"}, "exchange direction": "OUTPUT", "other": {"anies": [{"name": "referenceToUnitGroupDataSet", "value": {"shortDescription": [{"value": "kg", "lang": "de"}], "type": "unit group data set", "refObjectId": "ad38d542-3fe9-439d-9b95-2f5f7752acaf", "uri": "../unitgroups/ad38d542-3fe9-439d-9b95-2f5f7752acaf.xml"}}, {"value": "0", "module": "A1-A3"}, {"value": "0", "module": "A4"}, {"value": "0.0863293478112492", "module": "A5"}, {"value": "0", "module": "B2"}, {"value": "0", "module": "B3"}, {"value": "0", "module": "C1"}, {"value": "0", "module": "C2"}, {"value": "0", "module": "C3"}, {"value": "0", "module": "C4"}, {"value": "0", "module": "D"}]}, "resolvedFlowVersion": "38.00.000", "flowProperties": [], "typeOfFlow": "Other flow", "classification": {"classHierarchy": "Quantities / Environmental quantities / EPD EN 15804 / LCI indicators", "name": "GaBiCategories"}}, {"dataSetInternalID": 16, "referenceToFlowDataSet": {"shortDescription": [{"value": "Stoffe für die Energierückgewinnung (MER)", "lang": "de"}, {"value": "Materials for energy recovery (MER)", "lang": "en"}], "type": "flow data set", "refObjectId": "59a9181c-3aaf-46ee-8b13-2b3723b6e447", "uri": "../flows/59a9181c-3aaf-46ee-8b13-2b3723b6e447.xml"}, "exchange direction": "OUTPUT", "other": {"anies": [{"name": "referenceToUnitGroupDataSet", "value": {"shortDescription": [{"value": "kg", "lang": "de"}], "type": "unit group data set", "refObjectId": "ad38d542-3fe9-439d-9b95-2f5f7752acaf", "uri": "../unitgroups/ad38d542-3fe9-439d-9b95-2f5f7752acaf.xml"}}, {"value": "0", "module": "A1-A3"}, {"value": "0", "module": "A4"}, {"value": "0", "module": "A5"}, {"value": "0", "module": "B2"}, {"value": "1.9955777538632E-05", "module": "B3"}, {"value": "0", "module": "C1"}, {"value": "0.997788876931601", "module": "C2"}, {"value": "0", "module": "C3"}, {"value": "0", "module": "C4"}, {"value": "0", "module": "D"}]}, "resolvedFlowVersion": "38.00.000", "flowProperties": [], "typeOfFlow": "Other flow", "classification": {"classHierarchy": "Quantities / Environmental quantities / EPD EN 15804 / LCI indicators", "name": "GaBiCategories"}}, {"dataSetInternalID": 17, "referenceToFlowDataSet": {"shortDescription": [{"value": "Exportierte elektrische Energie (EEE)", "lang": "de"}, {"value": "Exported electrical energy (EEE)", "lang": "en"}], "type": "flow data set", "refObjectId": "4da0c987-2b76-40d6-9e9e-82a017aaaf29", "uri": "../flows/4da0c987-2b76-40d6-9e9e-82a017aaaf29.xml"}, "exchange direction": "OUTPUT", "other": {"anies": [{"name": "referenceToUnitGroupDataSet", "value": {"shortDescription": [{"value": "MJ", "lang": "de"}], "type": "unit group data set", "refObjectId": "93a60a57-a3c8-11da-a746-0800200c9a66", "uri": "../unitgroups/93a60a57-a3c8-11da-a746-0800200c9a66.xml"}}, {"value": "0", "module": "A1-A3"}, {"value": "0", "module": "A4"}, {"value": "0.111", "module": "A5"}, {"value": "0", "module": "B2"}, {"value": "2.8E-05", "module": "B3"}, {"value": "0", "module": "C1"}, {"value": "0", "module": "C2"}, {"value": "13.9", "module": "C3"}, {"value": "0", "module": "C4"}, {"value": "14.011028", "module": "D"}]}, "resolvedFlowVersion": "38.00.000", "flowProperties": [], "typeOfFlow": "Other flow", "classification": {"classHierarchy": "Quantities / Environmental quantities / EPD EN 15804 / LCI indicators", "name": "GaBiCategories"}}, {"dataSetInternalID": 18, "referenceToFlowDataSet": {"shortDescription": [{"value": "Exportierte thermische Energie (EET)", "lang": "de"}, {"value": "Exported thermal energy (EET)", "lang": "en"}], "type": "flow data set", "refObjectId": "98daf38a-7a79-46d3-9a37-2b7bd0955810", "uri": "../flows/98daf38a-7a79-46d3-9a37-2b7bd0955810.xml"}, "exchange direction": "OUTPUT", "other": {"anies": [{"name": "referenceToUnitGroupDataSet", "value": {"shortDescription": [{"value": "MJ", "lang": "de"}], "type": "unit group data set", "refObjectId": "93a60a57-a3c8-11da-a746-0800200c9a66", "uri": "../unitgroups/93a60a57-a3c8-11da-a746-0800200c9a66.xml"}}, {"value": "0", "module": "A1-A3"}, {"value": "0", "module": "A4"}, {"value": "0.198", "module": "A5"}, {"value": "0", "module": "B2"}, {"value": "5.26E-05", "module": "B3"}, {"value": "0", "module": "C1"}, {"value": "0", "module": "C2"}, {"value": "24.7", "module": "C3"}, {"value": "0", "module": "C4"}, {"value": "24.8980526", "module": "D"}]}, "resolvedFlowVersion": "38.00.000", "flowProperties": [], "typeOfFlow": "Other flow", "classification": {"classHierarchy": "Quantities / Environmental quantities / EPD EN 15804 / LCI indicators", "name": "GaBiCategories"}}]}, "LCIAResults": {"LCIAResult": [{"referenceToLCIAMethodDataSet": {"shortDescription": [{"value": "Globales Erwärmungspotenzial total (GWP-total)", "lang": "de"}, {"value": "Global Warming Potential total (GWP-total)", "lang": "en"}], "type": "LCIA method data set", "refObjectId": "6a37f984-a4b3-458a-a20a-64418c145fa2", "uri": "../lciamethods/6a37f984-a4b3-458a-a20a-64418c145fa2.xml"}, "other": {"anies": [{"name": "referenceToUnitGroupDataSet", "value": {"shortDescription": [{"value": "kg CO_(2)-Äq.", "lang": "de"}], "type": "unit group data set", "refObjectId": "1ebf3012-d0db-4de2-aefd-ef30cedb0be1", "uri": "../unitgroups/1ebf3012-d0db-4de2-aefd-ef30cedb0be1.xml"}}, {"value": "-4.65397131656596", "module": "A1-A3"}, {"value": "0.21097021602815", "module": "A4"}, {"value": "0.163158882404269", "module": "A5"}, {"value": "0.000476509063181356", "module": "B2"}, {"value": "0.00035866105164776", "module": "B3"}, {"value": "0", "module": "C1"}, {"value": "0.0483106930064387", "module": "C2"}, {"value": "10.384054765493", "module": "C3"}, {"value": "0", "module": "C4"}, {"value": "-2.92857242658584", "module": "D"}]}}, {"referenceToLCIAMethodDataSet": {"shortDescription": [{"value": "Globales Erwärmungspotenzial fossil (GWP-fossil)", "lang": "de"}, {"value": "Global Warming Potential fossil fuels (GWP-fossil)", "lang": "en"}], "type": "LCIA method data set", "refObjectId": "5f635281-343e-44fb-83df-1971b155e6b6", "uri": "../lciamethods/5f635281-343e-44fb-83df-1971b155e6b6.xml"}, "other": {"anies": [{"name": "referenceToUnitGroupDataSet", "value": {"shortDescription": [{"value": "kg CO_(2)-Äq.", "lang": "de"}], "type": "unit group data set", "refObjectId": "1ebf3012-d0db-4de2-aefd-ef30cedb0be1", "uri": "../unitgroups/1ebf3012-d0db-4de2-aefd-ef30cedb0be1.xml"}}, {"value": "5.5994880832524", "module": "A1-A3"}, {"value": "0.210387852642786", "module": "A4"}, {"value": "0.0531498490837624", "module": "A5"}, {"value": "0.000476457262856193", "module": "B2"}, {"value": "0.000358555057532151", "module": "B3"}, {"value": "0", "module": "C1"}, {"value": "0.0478646176598092", "module": "C2"}, {"value": "0.234028852407005", "module": "C3"}, {"value": "0", "module": "C4"}, {"value": "-2.92838058876033", "module": "D"}]}}, {"referenceToLCIAMethodDataSet": {"shortDescription": [{"value": "Globales Erwärmungspotenzial biogen (GWP-biogenic)", "lang": "de"}, {"value": "Global Warming Potential biogenic (GWP-biogenic)", "lang": "en"}], "type": "LCIA method data set", "refObjectId": "2356e1ab-0185-4db5-86e5-16de51c7485c", "uri": "../lciamethods/2356e1ab-0185-4db5-86e5-16de51c7485c.xml"}, "other": {"anies": [{"name": "referenceToUnitGroupDataSet", "value": {"shortDescription": [{"value": "kg CO_(2)-Äq.", "lang": "de"}], "type": "unit group data set", "refObjectId": "1ebf3012-d0db-4de2-aefd-ef30cedb0be1", "uri": "../unitgroups/1ebf3012-d0db-4de2-aefd-ef30cedb0be1.xml"}}, {"value": "-10.26", "module": "A1-A3"}, {"value": "0", "module": "A4"}, {"value": "0.11", "module": "A5"}, {"value": "0", "module": "B2"}, {"value": "0", "module": "B3"}, {"value": "0", "module": "C1"}, {"value": "0", "module": "C2"}, {"value": "10.15", "module": "C3"}, {"value": "0", "module": "C4"}, {"value": "0", "module": "D"}]}}, {"referenceToLCIAMethodDataSet": {"shortDescription": [{"value": "Globales Erwärmungspotenzial luluc (GWP-luluc)", "lang": "de"}, {"value": "Global Warming Potential luluc (GWP-luluc)", "lang": "en"}], "type": "LCIA method data set", "refObjectId": "4331bbdb-978a-490d-8707-eeb047f01a55", "uri": "../lciamethods/4331bbdb-978a-490d-8707-eeb047f01a55.xml"}, "other": {"anies": [{"name": "referenceToUnitGroupDataSet", "value": {"shortDescription": [{"value": "kg CO_(2)-Äq.", "lang": "de"}], "type": "unit group data set", "refObjectId": "1ebf3012-d0db-4de2-aefd-ef30cedb0be1", "uri": "../unitgroups/1ebf3012-d0db-4de2-aefd-ef30cedb0be1.xml"}}, {"value": "0.00654060018164214", "module": "A1-A3"}, {"value": "0.000582363385363913", "module": "A4"}, {"value": "9.03332050656533E-06", "module": "A5"}, {"value": "5.18003251633107E-08", "module": "B2"}, {"value": "1.0599411560908E-07", "module": "B3"}, {"value": "0", "module": "C1"}, {"value": "0.000446075346629441", "module": "C2"}, {"value": "2.59130860082584E-05", "module": "C3"}, {"value": "0", "module": "C4"}, {"value": "-0.000191837825507665", "module": "D"}]}}, {"referenceToLCIAMethodDataSet": {"shortDescription": [{"value": "Abbau Potential der stratosphärischen Ozonschicht (ODP)", "lang": "de"}, {"value": "Depletion potential of the stratospheric ozone layer (ODP)", "lang": "en"}], "type": "LCIA method data set", "refObjectId": "b5c629d6-def3-11e6-bf01-fe55135034f3", "uri": "../lciamethods/b5c629d6-def3-11e6-bf01-fe55135034f3.xml"}, "other": {"anies": [{"name": "referenceToUnitGroupDataSet", "value": {"shortDescription": [{"value": "kg CFC11-Äq.", "lang": "de"}], "type": "unit group data set", "refObjectId": "d9e957c9-7309-4474-bf3a-7777df6c4e5b", "uri": "../unitgroups/d9e957c9-7309-4474-bf3a-7777df6c4e5b.xml"}}, {"value": "3.37458437305924E-11", "module": "A1-A3"}, {"value": "1.82309171498896E-14", "module": "A4"}, {"value": "2.59621790013155E-15", "module": "A5"}, {"value": "8.79092899960663E-15", "module": "B2"}, {"value": "9.30903699639373E-16", "module": "B3"}, {"value": "0", "module": "C1"}, {"value": "6.26706005215435E-15", "module": "C2"}, {"value": "1.23151924341375E-12", "module": "C3"}, {"value": "0", "module": "C4"}, {"value": "-2.32299615944459E-11", "module": "D"}]}}, {"referenceToLCIAMethodDataSet": {"shortDescription": [{"value": "Versauerungspotenzial von Boden und Wasser (AP)", "lang": "de"}, {"value": "Acidification potential of land and water (AP)", "lang": "en"}], "type": "LCIA method data set", "refObjectId": "b5c611c6-def3-11e6-bf01-fe55135034f3", "uri": "../lciamethods/b5c611c6-def3-11e6-bf01-fe55135034f3.xml"}, "other": {"anies": [{"name": "referenceToUnitGroupDataSet", "value": {"shortDescription": [{"value": "mol H^(+)-Äq.", "lang": "de"}], "type": "unit group data set", "refObjectId": "42e089ac-92bf-4bf2-8ca1-5fc40d18f2ed", "uri": "../unitgroups/42e089ac-92bf-4bf2-8ca1-5fc40d18f2ed.xml"}}, {"value": "0.0180293510850983", "module": "A1-A3"}, {"value": "0.00542848418706531", "module": "A4"}, {"value": "9.81602866841548E-06", "module": "A5"}, {"value": "1.01763632005354E-06", "module": "B2"}, {"value": "6.99887913940115E-07", "module": "B3"}, {"value": "0", "module": "C1"}, {"value": "0.000405041650443886", "module": "C2"}, {"value": "0.00597619645196866", "module": "C3"}, {"value": "0", "module": "C4"}, {"value": "-0.00368159524710209", "module": "D"}]}}, {"referenceToLCIAMethodDataSet": {"shortDescription": [{"value": "Eutrophierungspotenzial Süßwasser (EP-freshwater)", "lang": "de"}, {"value": "Eutrophication potential aquatic freshwater (EP-freshwater)", "lang": "en"}], "type": "LCIA method data set", "refObjectId": "b53ec18f-7377-4ad3-86eb-cc3f4f276b2b", "uri": "../lciamethods/b53ec18f-7377-4ad3-86eb-cc3f4f276b2b.xml"}, "other": {"anies": [{"name": "referenceToUnitGroupDataSet", "value": {"shortDescription": [{"value": "kg P-Äq.", "lang": "de"}], "type": "unit group data set", "refObjectId": "0429039d-a61d-4590-ba67-aa4a20a810a1", "uri": "../unitgroups/0429039d-a61d-4590-ba67-aa4a20a810a1.xml"}}, {"value": "2.92119617189792E-05", "module": "A1-A3"}, {"value": "2.62367903052661E-07", "module": "A4"}, {"value": "4.1315421424082E-09", "module": "A5"}, {"value": "1.86276263995748E-09", "module": "B2"}, {"value": "6.55161586972638E-10", "module": "B3"}, {"value": "0", "module": "C1"}, {"value": "1.76095737777913E-07", "module": "C2"}, {"value": "3.21089625667921E-07", "module": "C3"}, {"value": "0", "module": "C4"}, {"value": "-4.79079936886513E-06", "module": "D"}]}}, {"referenceToLCIAMethodDataSet": {"shortDescription": [{"value": "Eutrophierungspotenzial Salzwasser (EP-marine)", "lang": "de"}, {"value": "Eutrophication potential aquatic marine (EP-marine)", "lang": "en"}], "type": "LCIA method data set", "refObjectId": "b5c619fa-def3-11e6-bf01-fe55135034f3", "uri": "../lciamethods/b5c619fa-def3-11e6-bf01-fe55135034f3.xml"}, "other": {"anies": [{"name": "referenceToUnitGroupDataSet", "value": {"shortDescription": [{"value": "kg N-Äq.", "lang": "de"}], "type": "unit group data set", "refObjectId": "d05bb823-ecdf-4686-8c40-bf1d9257859f", "uri": "../unitgroups/d05bb823-ecdf-4686-8c40-bf1d9257859f.xml"}}, {"value": "0.0090169681404074", "module": "A1-A3"}, {"value": "0.00133565367342965", "module": "A4"}, {"value": "3.30118961604238E-06", "module": "A5"}, {"value": "2.4380265082922E-07", "module": "B2"}, {"value": "1.66146011334883E-07", "module": "B3"}, {"value": "0", "module": "C1"}, {"value": "0.000201940082391265", "module": "C2"}, {"value": "0.00283755416943098", "module": "C3"}, {"value": "0", "module": "C4"}, {"value": "-0.00107436959331386", "module": "D"}]}}, {"referenceToLCIAMethodDataSet": {"shortDescription": [{"value": "Eutrophierungspotenzial Land (EP-terrestrial)", "lang": "de"}, {"value": "Eutrophication potential terrestrial (EP-terrestrial)", "lang": "en"}], "type": "LCIA method data set", "refObjectId": "b5c614d2-def3-11e6-bf01-fe55135034f3", "uri": "../lciamethods/b5c614d2-def3-11e6-bf01-fe55135034f3.xml"}, "other": {"anies": [{"name": "referenceToUnitGroupDataSet", "value": {"shortDescription": [{"value": "mol N-Äq.", "lang": "de"}], "type": "unit group data set", "refObjectId": "71b4d617-0ec9-4d3f-b65e-e438940c2401", "uri": "../unitgroups/71b4d617-0ec9-4d3f-b65e-e438940c2401.xml"}}, {"value": "0.072508367258659", "module": "A1-A3"}, {"value": "0.014655431315605", "module": "A4"}, {"value": "4.90494061409678E-05", "module": "A5"}, {"value": "2.54414885840827E-06", "module": "B2"}, {"value": "1.81230130836953E-06", "module": "B3"}, {"value": "0", "module": "C1"}, {"value": "0.00222978729061019", "module": "C2"}, {"value": "0.0328494744626601", "module": "C3"}, {"value": "0", "module": "C4"}, {"value": "-0.0115002455923992", "module": "D"}]}}, {"referenceToLCIAMethodDataSet": {"shortDescription": [{"value": "Bildungspotential für troposphärisches Ozon (POCP)", "lang": "de"}, {"value": "Formation potential of tropospheric ozone photochemical oxidants (POCP)", "lang": "en"}], "type": "LCIA method data set", "refObjectId": "b5c610fe-def3-11e6-bf01-fe55135034f3", "uri": "../lciamethods/b5c610fe-def3-11e6-bf01-fe55135034f3.xml"}, "other": {"anies": [{"name": "referenceToUnitGroupDataSet", "value": {"shortDescription": [{"value": "kg NMVOC-Äq.", "lang": "de"}], "type": "unit group data set", "refObjectId": "d27c25f8-fbc1-44c6-b47b-4adbae4199c6", "uri": "../unitgroups/d27c25f8-fbc1-44c6-b47b-4adbae4199c6.xml"}}, {"value": "0.0183422384482377", "module": "A1-A3"}, {"value": "0.00369515983941264", "module": "A4"}, {"value": "7.47251458007668E-06", "module": "A5"}, {"value": "6.49572425227571E-07", "module": "B2"}, {"value": "6.21596471519032E-07", "module": "B3"}, {"value": "0", "module": "C1"}, {"value": "0.000379234562020575", "module": "C2"}, {"value": "0.00730533373292902", "module": "C3"}, {"value": "0", "module": "C4"}, {"value": "-0.00299205340787278", "module": "D"}]}}, {"referenceToLCIAMethodDataSet": {"shortDescription": [{"value": "Potenzial für den abiotischen Abbau nicht fossiler Ressourcen (ADPE)", "lang": "de"}, {"value": "Abiotic depletion potential for non fossil resources (ADPE)", "lang": "en"}], "type": "LCIA method data set", "refObjectId": "b2ad6494-c78d-11e6-9d9d-cec0c932ce01", "uri": "../lciamethods/b2ad6494-c78d-11e6-9d9d-cec0c932ce01.xml"}, "other": {"anies": [{"name": "referenceToUnitGroupDataSet", "value": {"shortDescription": [{"value": "kg Sb-Äq.", "lang": "de"}], "type": "unit group data set", "refObjectId": "54ccd2d9-a32a-4fc2-923d-f2c8c93e89d4", "uri": "../unitgroups/54ccd2d9-a32a-4fc2-923d-f2c8c93e89d4.xml"}}, {"value": "5.44479281821588E-07", "module": "A1-A3"}, {"value": "5.49965553226358E-09", "module": "A4"}, {"value": "8.72734846079844E-11", "module": "A5"}, {"value": "7.36837806845335E-11", "module": "B2"}, {"value": "1.571902784454E-09", "module": "B3"}, {"value": "0", "module": "C1"}, {"value": "3.1933536681919E-09", "module": "C2"}, {"value": "1.16204085655058E-08", "module": "C3"}, {"value": "0", "module": "C4"}, {"value": "-2.12018103733061E-07", "module": "D"}]}}, {"referenceToLCIAMethodDataSet": {"shortDescription": [{"value": "Potenzial für den abiotischen Abbau fossiler Brennstoffe (ADPF)", "lang": "de"}, {"value": "Abiotic depletion potential for fossil resources (ADPF)", "lang": "en"}], "type": "LCIA method data set", "refObjectId": "b2ad6110-c78d-11e6-9d9d-cec0c932ce01", "uri": "../lciamethods/b2ad6110-c78d-11e6-9d9d-cec0c932ce01.xml"}, "other": {"anies": [{"name": "referenceToUnitGroupDataSet", "value": {"shortDescription": [{"value": "MJ", "lang": "de"}], "type": "unit group data set", "refObjectId": "93a60a57-a3c8-11da-a746-0800200c9a66", "uri": "../unitgroups/93a60a57-a3c8-11da-a746-0800200c9a66.xml"}}, {"value": "120.829815155752", "module": "A1-A3"}, {"value": "2.65415865417434", "module": "A4"}, {"value": "0.0194141426251172", "module": "A5"}, {"value": "0.010026065888016", "module": "B2"}, {"value": "0.0104729502601776", "module": "B3"}, {"value": "0", "module": "C1"}, {"value": "0.65612462678144", "module": "C2"}, {"value": "3.6705533427394", "module": "C3"}, {"value": "0", "module": "C4"}, {"value": "-54.1421749039589", "module": "D"}]}}, {"referenceToLCIAMethodDataSet": {"shortDescription": [{"value": "Wassernutzung (WDP)", "lang": "de"}, {"value": "Water use (WDP)", "lang": "en"}], "type": "LCIA method data set", "refObjectId": "b2ad66ce-c78d-11e6-9d9d-cec0c932ce01", "uri": "../lciamethods/b2ad66ce-c78d-11e6-9d9d-cec0c932ce01.xml"}, "other": {"anies": [{"name": "referenceToUnitGroupDataSet", "value": {"shortDescription": [{"value": "m^(3) Welt-Äq. entzogen", "lang": "de"}], "type": "unit group data set", "refObjectId": "6ae2df01-888e-46c8-b17d-49fa3869b476", "uri": "../unitgroups/6ae2df01-888e-46c8-b17d-49fa3869b476.xml"}}, {"value": "0.628063081737662", "module": "A1-A3"}, {"value": "0.00100226026147585", "module": "A4"}, {"value": "0.00482482266383088", "module": "A5"}, {"value": "0.000106190472769002", "module": "B2"}, {"value": "2.48240909334552E-05", "module": "B3"}, {"value": "0", "module": "C1"}, {"value": "0.000582011689955988", "module": "C2"}, {"value": "1.26073742557426", "module": "C3"}, {"value": "0", "module": "C4"}, {"value": "-0.281434182536937", "module": "D"}]}}, {"referenceToLCIAMethodDataSet": {"shortDescription": [{"value": "Auftreten von Krankheiten aufgrund von Feinstaubemissionen (PM)", "lang": "de"}, {"value": "Incidence of disease due to PM emissions (PM)", "lang": "en"}], "type": "LCIA method data set", "refObjectId": "b5c602c6-def3-11e6-bf01-fe55135034f3", "uri": "../lciamethods/b5c602c6-def3-11e6-bf01-fe55135034f3.xml"}, "other": {"anies": [{"name": "referenceToUnitGroupDataSet", "value": {"shortDescription": [{"value": "Krankheitsfälle", "lang": "de"}], "type": "unit group data set", "refObjectId": "3883559b-648f-4afc-8ba2-0bd24f3affa3", "uri": "../unitgroups/3883559b-648f-4afc-8ba2-0bd24f3affa3.xml"}}, {"module": "A1-A3"}, {"module": "A4"}, {"module": "A5"}, {"module": "B2"}, {"module": "B3"}, {"module": "C1"}, {"module": "C2"}, {"module": "C3"}, {"module": "C4"}, {"module": "D"}]}}, {"referenceToLCIAMethodDataSet": {"shortDescription": [{"value": "Wirkung durch Exposition des Menschen mit U235 (IR)", "lang": "de"}, {"value": "Human exposure efficiency relative to U235 (IR)", "lang": "en"}], "type": "LCIA method data set", "refObjectId": "b5c632be-def3-11e6-bf01-fe55135034f3", "uri": "../lciamethods/b5c632be-def3-11e6-bf01-fe55135034f3.xml"}, "other": {"anies": [{"name": "referenceToUnitGroupDataSet", "value": {"shortDescription": [{"value": "kBq U235-Äq.", "lang": "de"}], "type": "unit group data set", "refObjectId": "456b05bf-1415-44a9-9993-02452f554c09", "uri": "../unitgroups/456b05bf-1415-44a9-9993-02452f554c09.xml"}}, {"module": "A1-A3"}, {"module": "A4"}, {"module": "A5"}, {"module": "B2"}, {"module": "B3"}, {"module": "C1"}, {"module": "C2"}, {"module": "C3"}, {"module": "C4"}, {"module": "D"}]}}, {"referenceToLCIAMethodDataSet": {"shortDescription": [{"value": "Toxizitätsvergleichseinheit für Ökosysteme (ETP-fw)", "lang": "de"}, {"value": "Comparative toxic unit for ecosystems (ETP-fw)", "lang": "en"}], "type": "LCIA method data set", "refObjectId": "ee1082d1-b0f7-43ca-a1f0-21e2a4a74511", "uri": "../lciamethods/ee1082d1-b0f7-43ca-a1f0-21e2a4a74511.xml"}, "other": {"anies": [{"name": "referenceToUnitGroupDataSet", "value": {"shortDescription": [{"value": "CTUe", "lang": "de"}], "type": "unit group data set", "refObjectId": "aa959ded-f1eb-4efb-9c5c-2d60be36b3e6", "uri": "../unitgroups/aa959ded-f1eb-4efb-9c5c-2d60be36b3e6.xml"}}, {"module": "A1-A3"}, {"module": "A4"}, {"module": "A5"}, {"module": "B2"}, {"module": "B3"}, {"module": "C1"}, {"module": "C2"}, {"module": "C3"}, {"module": "C4"}, {"module": "D"}]}}, {"referenceToLCIAMethodDataSet": {"shortDescription": [{"value": "Toxizitätsvergleichseinheit für Menschen (krebserregend) (HTP-c)", "lang": "de"}, {"value": "Comparative toxic unit for humans (carcinogenic) (HTP-c)", "lang": "en"}], "type": "LCIA method data set", "refObjectId": "2299222a-bbd8-474f-9d4f-4dd1f18aea7c", "uri": "../lciamethods/2299222a-bbd8-474f-9d4f-4dd1f18aea7c.xml"}, "other": {"anies": [{"name": "referenceToUnitGroupDataSet", "value": {"shortDescription": [{"value": "CTUh", "lang": "de"}], "type": "unit group data set", "refObjectId": "d4c9523e-2d7e-49fd-8469-998f547d3a70", "uri": "../unitgroups/d4c9523e-2d7e-49fd-8469-998f547d3a70.xml"}}, {"module": "A1-A3"}, {"module": "A4"}, {"module": "A5"}, {"module": "B2"}, {"module": "B3"}, {"module": "C1"}, {"module": "C2"}, {"module": "C3"}, {"module": "C4"}, {"module": "D"}]}}, {"referenceToLCIAMethodDataSet": {"shortDescription": [{"value": "Toxizitätsvergleichseinheit für Menschen (nicht krebserregend) (HTP-nc)", "lang": "de"}, {"value": "Comparative toxic unit for humans (noncarcinogenic) (HTP-nc)", "lang": "en"}], "type": "LCIA method data set", "refObjectId": "3af763a5-b7a1-48c9-9cee-1f223481fcef", "uri": "../lciamethods/3af763a5-b7a1-48c9-9cee-1f223481fcef.xml"}, "other": {"anies": [{"name": "referenceToUnitGroupDataSet", "value": {"shortDescription": [{"value": "CTUh", "lang": "de"}], "type": "unit group data set", "refObjectId": "d4c9523e-2d7e-49fd-8469-998f547d3a70", "uri": "../unitgroups/d4c9523e-2d7e-49fd-8469-998f547d3a70.xml"}}, {"module": "A1-A3"}, {"module": "A4"}, {"module": "A5"}, {"module": "B2"}, {"module": "B3"}, {"module": "C1"}, {"module": "C2"}, {"module": "C3"}, {"module": "C4"}, {"module": "D"}]}}, {"referenceToLCIAMethodDataSet": {"shortDescription": [{"value": "Bodenqualitätsindex (SQP)", "lang": "de"}, {"value": "Soil quality index (SQP)", "lang": "en"}], "type": "LCIA method data set", "refObjectId": "b2ad6890-c78d-11e6-9d9d-cec0c932ce01", "uri": "../lciamethods/b2ad6890-c78d-11e6-9d9d-cec0c932ce01.xml"}, "other": {"anies": [{"name": "referenceToUnitGroupDataSet", "value": {"shortDescription": [{"value": "SQP", "lang": "de"}], "type": "unit group data set", "refObjectId": "f130951c-e67f-4f7f-8dd4-665de3974e18", "uri": "../unitgroups/f130951c-e67f-4f7f-8dd4-665de3974e18.xml"}}, {"module": "A1-A3"}, {"module": "A4"}, {"module": "A5"}, {"module": "B2"}, {"module": "B3"}, {"module": "C1"}, {"module": "C2"}, {"module": "C3"}, {"module": "C4"}, {"module": "D"}]}}]}, "otherAttributes": {"{http://www.indata.network/EPD/2019}epd-version": "1.2"}, "version": "1.1", "locations": "../ILCDLocations.xml"}