{"processInformation": {"dataSetInformation": {"UUID": "3a9b06e9-50a1-44a3-b923-6b66b89d16e0", "name": {"baseName": [{"value": "Steel pipe", "lang": "en"}, {"value": "Stahlrohr", "lang": "de"}], "functionalUnitFlowProperties": [{"value": "Steel pipe", "lang": "en"}]}, "classificationInformation": {"classification": [{"class": [{"value": "Gebäudetechnik", "level": 0, "classId": "8"}, {"value": "Heizung", "level": 1, "classId": "8.1"}, {"value": "Wärmeverteilung und Abgabe", "level": 2, "classId": "8.1.02"}], "name": "oekobau.dat"}]}, "generalComment": [{"value": "This data set has been modeled according to the European Standard EN 15804+A2 for Sustainable Building. Results are depicted in modules that allow the structured expression of results over the entire life cycle.", "lang": "en"}, {"value": "Dieser Datensatz wurde nach dem European Standard EN 15804+A2 für Nachhaltiges Bauen modelliert. Ergebnisse werden in Modulen abgebildet, die den strukturierten Ausdruck von Ergebnissen über den gesamten Lebenszyklus zulassen.", "lang": "de"}], "other": {"anies": [{"margins": 10, "description": [{"value": "Product system almost completely covered. Good technological, temporal and geographic representativeness.", "lang": "en"}, {"value": "Produktsystem weitgehend vollständig abgebildet. Gute technologische, zeitliche und geographische Repräsentativität.", "lang": "de"}]}]}}, "quantitativeReference": {"referenceToReferenceFlow": [101140], "type": "Reference flow(s)"}, "time": {"referenceYear": 2023, "dataSetValidUntil": 2026, "timeRepresentativenessDescription": [{"value": "Annual average", "lang": "en"}, {"value": "Jährlicher Durchschnitt", "lang": "de"}]}, "geography": {"locationOfOperationSupplyOrProduction": {"descriptionOfRestrictions": [{"value": "The data set represents the country specific situation in Germany, focusing on the main technologies, the region specific characteristics and / or import statistics.", "lang": "en"}, {"value": "Der Datensatz bildet die länderspezifische Situation in Deutschland ab. Dabei werden Haupttechnologien, spezifische regionale Charakteristiken und ggf. Importstatistiken berücksichtigt.", "lang": "de"}], "location": "DE"}}, "technology": {"technologyDescriptionAndIncludedProcesses": [{"value": "Steel pipe for the installation of heatings and gas supply. According to VDI guideline 2067 for steel pipes an average life span of 40 years can be assumed for heating, gas supply and cold water and 25 years for warm water. Steel production: The preparation of the iron ore includes mainly the crushing. The average iron content in the iron ore is 60%. Pellets are small crystallized balls of iron ore. The pelletisation process consists of grinding and drying, balling and induration followed by screening and handling. The provision of hard coal is described in the respective documentation file (please see link below).  For every fraction the transport to Germany is considered in the data set. The transportation includes all necessary transportation means like ship and where required railway.  The coke oven produces as main product coke out of hard coal. The main by-product resulting from this operation is coke oven gas (COG gas) which is used as energy carrier within the steel production. Further by-products as tar, benzene and sulphur are sold and therefore excluded from the system by allocation to (net) calorific value.  In the sinter plant sinter feed is produced based on the major inputs coke, iron ore and additives. Sintering is an agglomeration process which takes place under high temperatures. The raw materials (fine iron ore, coke breeze, additives) are blended, then the coke breeze is ignited. The result of the sinter process is the so-called sinter cake which has to be broken up, screened and cooled down.  The blast furnace is a closed system into which iron bearing materials (iron ore lump, sinter and / or pellets), additives (slag formers such as limestone) and reducing agents (coke) are continuously fed from the top of the furnace shaft through a charging system. A hot air blast, enriched with oxygen and auxiliary reducing agents (e.g. pulverized coal) is injected providing a counter-current of reducing gases. The air blast reacts with the reducing agents to produce mainly carbon monoxide which in turn reduces iron oxides to metal iron. The main products of the blast furnace operation are hot metal, blast furnace gas (BF gas) and blast furnace slag (BF slag). The BF gas is used as fuel for heating comparable to the COG gas or for electricity production.  The objective in oxygen steelmaking is to burn (i.e., oxidise) the undesirable impurities contained in the metallic feedstock. The main elements thus converted into oxides are carbon, silicon, manganese, phosphorus and sulphur. The purpose of this oxidation process, therefore, are to reduce the carbon content to a specified level to adjust the contents of desirable foreign elements and to remove undesirable impurities to the greatest possible extent. The production of steel by the basic oxygen furnace (BOF) process is a discontinuous process which involves the following steps: transfer and storage of hot metal, pre-treatment of hot metal (desulphurisation), oxidation in the BOF (decarburisation and oxidation of impurities) and secondary metallurgical treatment (e.g. vacuum treatment and adding alloying elements). Within the main step of the oxygen steelmaking, the hot metal feeds together with steel scrap the converter. The main products of the converter are the liquid steel, the converter gas or basic oxygen furnace gas (BOF gas) and the BOF slag. The gas is as well used as energy carrier within the steel production.  Afterwards the continuous casting takes place whereby the liquid steel is cast in continuous strand. The output of the continuous casting process is the slab.  The following operations are two rolling processes: the hot strip mill and the cold rolling mill. In the hot rolling mill the slab is reshaped above the recrystallization temperature. The qualities obtained in this process are e.g. strength and surface quality. During the rolling process the material passes through the furnace and the rolling line. In the furnace the metal is preheated by natural gas. There is no need for an additional warming, if the hot slabs are directly charged into the rolling mill. The forming is done in various rolling frames until the final shape is obtained. The steel scrap in this process are directly recycled.  In the cold rolling mill the material is reshaped below the recrystallization temperature. Thereby a enhanced surface quality, an improved dimensional accuracy as well as a higher strength are achieved. The different process steps are: pickling, the rolling line and the heat treatment.  The cold rolled sheet is transferred to the hot-dip galvanising. The zinc coating is applied by dipping the sheet steel into a hot zinc bath. During the hot-dip galvanising the cold rolled sheet passes the following process steps: preheating furnace (organic impurities are burned off), reduction zone (the sheet is heated to cause recrystallization), cooling and homogenization as well as metal bath (coating of the sheet)  and finishing stand.\nBackground system:\nElectricity: Electricity is modelled according to the individual country-specific situations. The country-specific modelling is achieved on multiple levels. Firstly, individual energy carrier specific power plants and plants for renewable energy sources are modelled according to the current national electricity grid mix. Modelling the electricity consumption mix includes transmission / distribution losses and the own use by energy producers (own consumption of power plants and \"other\" own consumption e.g. due to pumped storage hydro power etc.), as well as imported electricity. Secondly, the national emission and efficiency standards of the power plants are modelled as well as the share of electricity plants and combined heat and power plants (CHP). Thirdly, the country-specific energy carrier supply (share of imports and / or domestic supply) including the country-specific energy carrier properties (e.g. element and energy content) are accounted for. Fourthly, the exploration, mining/production, processing and transport processes of the energy carrier supply chains are modelled according to the specific situation of each electricity producing country. The different production and processing techniques (emissions and efficiencies) in the different energy producing countries are considered, e.g. different crude oil production technologies or different flaring rates at the oil platforms.\nThermal energy, process steam: The thermal energy and process steam supply is modelled according to the individual country-specific situation with regard to emission standards and considered energy carriers. The thermal energy and process steam are produced at heat plants. Efficiencies for thermal energy production are by definition 100% in relation to the corresponding energy carrier input. For process steam the efficiency ranges from 85%, 90% to 95%. The energy carriers used for the generation of thermal energy and process steam are modelled according to the specific import situation (see electricity above).\nTransports: All relevant and known transport processes are included. Ocean-going and inland ship transport as well as rail, truck and pipeline transport of bulk commodities are considered.\nEnergy carriers: The energy carriers are modelled according to the specific supply situation (see electricity above).\nRefinery products: Diesel fuel, gasoline, technical gases, fuel oils, lubricants and residues such as bitumen are modelled with a parameterised country-specific refinery model. The refinery model represents the current national standard in refining techniques (e.g. emission level, internal energy consumption, etc.) as well as the individual country-specific product output spectrum, which can be quite different from country to country. The supply of crude oil is modelled, again, according to the country-specific situation with the respective properties of the resources.", "lang": "en"}, {"value": "Die Ökobilanz bezieht sich auf Stahlrohre für die Verwendung in Heizungen und Gasleitungen. Nach VDI-Richtlinie 2067 gilt für Stahlrohre in Heizungen sowie zur Gas- und Wasserdurchleitung eine Lebensdauer von 40 Jahren, für Leitungen zur Warmwasserführung wird eine Lebensdauer von 25 Jahren veranschlagt. \nZur Stahlproduktion: Das Eisenerz als Basismaterial zur Stahlproduktion wird aufbereitet. In diesem Zusammenhang ist die Zerkleinerung und deren Energieaufwendung umweltseitig relevant. Der durchschnittliche Eisengehalt im Erz beträgt 60%. Als Zwischenprodukt auf dem Weg zum Stahl werden Eisenerzkügelchen (Pellets) erzeugt. Der Pelletierungsprozess besteht aus Mahlung, Trocknung, eigentlicher Pelletierung und Härtung. Die entstandenen Pellets werden anschließend gesiebt und aufbereitet. Die Dokumentation der Steinkohlegewinnung ist angehängt (siehe Link). Der Rohstofftransport  ist für jedes Vorprodukt im Datensatz enthalten. Die Beförderung schließt neben LKW-, auch den Schiffs- und Bahntransport ein, soweit benötigt. Die Kokerei produziert als Hauptprodukt Koks aus Steinkohle. Als hauptsächliches Nebenprodukt fällt in der Kokerei Koksofengas (COG-Gas) an, das als Energieträger im Stahlwerk genutzt wird. Als weitere Nebenprodukte entstehen Teer, Benzol und Schwefel. Diese werden verkauft und verlassen das betrachtete System. Die Lastenverteilung erfolgt auf der Basis des unteren Heizwertes. In der Sinteranlage wird auf Basis von Koks, Eisenerz und Zusatzstoffen Sintermaterial hergestellt. Sintern ist ein Agglomerationsverfahren, das bei hohen Temperaturen stattfindet. Zuerst werden die Rohstoffe (Feineisenerz, Koks, Zusatzstoffe) gemischt und das Koks entzündet. Das Produkt des Sinterprozesses ist der sogenannte Sinterkuchen, der anschließend gebrochen, gesiebt und abgekühlt wird. Im Hochofen wird das eisenhaltige Material (Eisenerzklumpen, sintermaterial und Pellets) sowie Zusatzstoffe (z. B. Kalkstein als Schlackenbildner) und Reduktionsmittel (Koks) kontinuierlich von der Spitze des Ofenschachtes eingespeist. Ein Heißluftstrom, der zusätzlich mit Sauerstoff und Reduktionsmitteln (z. B. Kohlenstaub) versetzt ist, wirkt der Bildung reduzierender Gase entgegen. Der Sauerstoff reagiert mit den Reduktionsmitteln hauptsächlich zu Kohlenmonoxid. Dieses reduziert wiederum Eisenoxide, um Eisen zu erhalten. Hauptprodukt des Hochofenbetriebes ist Roheisen, als Nebenprodukte fallen Hochofengas und Hochofenschlacke an. Das Gas wird zur Beheizung oder Stromerzeugung im Werk genutzt. \nDas Sauerstoffblasverfahren, der nächste Schritt in der Stahlherstellung, dient zur Entfernung unerwünschter Verunreinigungen aus dem Roheisen. Die hauptsächlich in Oxide umgewandelten Elemente sind Kohlenstoff, Silizium, Mangan, Phosphor und Schwefel. Der Kohlenstoffgehalt soll auf ein bestimmtes Niveau reduziert werden, um den Gehalt erwünschter Stoffe anzupassen und unerwünschte Verunreinigungen weitestgehend zu entfernen. Die Herstellung von Stahl durch den Sauerstoffaufblas-Konverter ist ein diskontinuierliches Verfahren, das folgende Prozessschritte beinhaltet: den Transfer des heißen Roheisens, die Vorbehandlung (z. B. Entschwefelung), die Oxidation im Konverter durch Entkohlung und Oxidation von Verunreinigungen und die sekundäre metallurgische Behandlung, z. B. durch Vakuum-Behandlung und Zugabe von Legierungselementen. Eingespeist wird sowohl Primär- als auch Sekundärmetall. Hauptprodukt des Konverterprozesses ist flüssiger Stahl. Außerdem entstehen Konvertergase und Schlacke. Das Gas wird zur Energieerzeugung in der Stahlproduktion genutzt.\nAls nächster Schritt zum fertigen Stahlprodukt erfolgt das Stranggießen. Hier wird flüssiger Stahl zu einem kontinuierlichen Strang gegossen und anschließend geteilt, um Brammen zu erzeugen.\nDer darauffolgende Walzprozess wird unterschieden nach Kalt- und Warmwalzverfahren. Beim Warmwalzen werden die Brammen oberhalb der Rekristallisationstemperatur verformt, um die Festigkeit und Oberflächenqualität zu verbessern. Das Metall wird dabei mittels Erdgas vorgewärmt. Dies ist nicht notwendig, wenn die noch heißen Brammen aus dem Konverterprozess direkt in das Walzwerk gelangen. Das Formen erfolgt über verschiedene Walzgerüste, bis die endgültige Dicke und Ausformung erreicht ist. Oft werden sogenannte Coils (Rollen, Spulen) erzeugt, die anschließend im Kaltwalzverfahren weiterverarbeitet werden. Anfallender Stahlschrott kann direkt recycelt werden. Das Kaltwalzen erfolgt unterhalb der Rekristallisationstemperatur bei Temperaturen um die 20°C. Dadurch kann eine bessere Oberflächenqualität, eine bessere Maßgenauigkeit und höhere Festigkeit erzielt werden als beim Warmwalzverfahren. Das Vormaterial wird zuerst von Rost und Zunder befreit. Das geschieht in den Verfahrensschritten Streckbiegen und Beizen. Das Streckbiegen bricht grobe Zunderschichten, Säuren entfernen Verunreinigungen der Bandoberfläche. Anschließend erfolgt das eigentliche Walzen. Oft ist dennoch eine zeitweise Wärmebehandlung, das sogenannte Zwischenglühen, notwendig, um die Kaltverfestigung des Metalls zu beseitigen.\nDas kaltgewalzte fertige Blech wird anschließend feuerverzinkt. Die Zinkbeschichtung wird durch Eintauchen in ein heißes Zinkbad aufgebracht. Beim Feuerverzinken durchläuft das Blech folgende Verarbeitungsschritte: 1. Vorwärmofen (Abbrennen organischer Verunreinigungen), 2. Reduktionszone (Erhitzung, um Rekristallisation auszulösen), 3. Kühlung und Homogenisierung sowie 4. Beschichtung im Metallbad und Fertiggerüst. \n\n\nEs wurde davon ausgegangen, dass große Geräte wie Heizkessel, Klima- und Lüftungsanlagen oder Fahrstühle zu 95% einem Recycling zugeführt werden. Für Rohre oder Kabel, die oft unterputzt sind wurde eine Recyclingrate von 90% angenommen. Die Recyclingquoten beziehen sich ausschließlich auf Metalle und Kunststoffe. Für mineralische Materialien wie Mineralwolle, Beton oder Keramik wurde eine Ablagerung auf einer Inertstoffdeponie angenommen. Es wurde angenommen das der Anteil an Metallen und Kunststoffen, der nicht einem Recycling zugeführt wird (5-10%) ebenfalls auf einer Inertstoffdeponie entsorgt wird (z.B. Kabelreste oder Rohrstücke im Bauschutt). Für die Kunststoffe wird davon ausgegangen, dass aufgrund der oft langen Lebensdauer und den verbundenen Verunreinigung nicht von einer stofflichen Verwertung ausgegangen werden kann und daher die Kunststoffe einer energetischen Verwertung in Müllverbrennungsanlagen (MVA) zugeführt werden. Für die Müllverbrennung wurde ein MVA-Modell mit durchschnittlichen europäischen Emissionswerten und Energieproduktion verwendet. In Abhängigkeit des zu verbrennenden Kunststoffes wurden unterschiedliche Prozesse mit den entsprechenden Elementarzusammensetzungen verwendet. Die Datensätze wurden in Zusammenarbeit mit der Confederation of European Waste-to-Energy Plants (CEWEP) erstellt und sind auf der Homepage der European Platform on LCA [EC 2008] verfügbar. Der aus der Kunststoffverbrennung erzeugte Strom sowie die erzeugte thermische Energie wurden mit dem europäischen Strom-bzw. Wärmemix gutgeschrieben. Die Gutschriften für das Recycling von Metallen oder der energetischen Verwertung von Kunststoffen, sowie die mit der Verwertung verbundenen Emissionen und Ressourcenverbräuche (Energie für Einschmelzen, Verbrennungsemissionen, Deponie) sind in den Datensätzen enthalten. Bei Materialen aus Eisen (Stahlbleche, Rohre, Grauguss) werden bei der Herstellung der Materialien bereits unterschiedliche Mengen an Stahlschrott eingesetzt. Diese Mengen wurden der recycelten Stahlmenge vor Zuführung in die Einschmelzung abgezogen, um keine Überwertung der Gutschriften zu erzeugen. Die Gutschrift wurde dann entsprechend mit primärem Stahl durchgeführt. Gutschriften für das Recycling von seltenen Erden oder Quecksilberemissionen aus Leuchtstofflampen konnten wegen fehlenden Daten nicht berücksichtigt werden. Es wurde davon ausgegangen, dass große Geräte wie Heizkessel, Klima- und Lüftungsanlagen oder Fahrstühle zu 95% einem Recycling zugeführt werden. Für Rohre oder Kabel, die oft unterputzt sind wurde eine Recyclingrate von 90% angenommen. Die Recyclingquoten beziehen sich ausschließlich auf Metalle und Kunststoffe. Für mineralische Materialien wie Mineralwolle, Beton oder Keramik wurde eine Ablagerung auf einer Inertstoffdeponie angenommen. Es wurde angenommen das der Anteil an Metallen und Kunststoffen, der nicht einem Recycling zugeführt wird (5-10%) ebenfalls auf einer Inertstoffdeponie entsorgt wird (z.B. Kabelreste oder Rohrstücke im Bauschutt). Für die Kunststoffe wird davon ausgegangen, dass aufgrund der oft langen Lebensdauer und den verbundenen Verunreinigung nicht von einer stofflichen Verwertung ausgegangen werden kann und daher die Kunststoffe einer energetischen Verwertung in Müllverbrennungsanlagen (MVA) zugeführt werden. Für die Müllverbrennung wurde ein MVA-Modell mit durchschnittlichen europäischen Emissionswerten und Energieproduktion verwendet. In Abhängigkeit des zu verbrennenden Kunststoffes wurden unterschiedliche Prozesse mit den entsprechenden Elementarzusammensetzungen verwendet. Die Datensätze wurden in Zusammenarbeit mit der Confederation of European Waste-to-Energy Plants (CEWEP) erstellt und sind auf der Homepage der European Platform on LCA [EC 2008] verfügbar. Der aus der Kunststoffverbrennung erzeugte Strom sowie die erzeugte thermische Energie wurden mit dem europäischen Strom-bzw. Wärmemix gutgeschrieben. Die Gutschriften für das Recycling von Metallen oder der energetischen Verwertung von Kunststoffen, sowie die mit der Verwertung verbundenen Emissionen und Ressourcenverbräuche (Energie für Einschmelzen, Verbrennungsemissionen, Deponie) sind in den Datensätzen enthalten. Bei Materialen aus Eisen (Stahlbleche, Rohre, Grauguss) werden bei der Herstellung der Materialien bereits unterschiedliche Mengen an Stahlschrott eingesetzt. Diese Mengen wurden der recycelten Stahlmenge vor Zuführung in die Einschmelzung abgezogen, um keine Überwertung der Gutschriften zu erzeugen. Die Gutschrift wurde dann entsprechend mit primärem Stahl durchgeführt. Gutschriften für das Recycling von seltenen Erden oder Quecksilberemissionen aus Leuchtstofflampen konnten wegen fehlenden Daten nicht berücksichtigt werden. \n\n\nHintergrundsystem:\nStrom: Die Stromerzeugung wird entsprechend der länderspezifischen Randbedingungen modelliert. Die landesspezifische Analyse beinhaltet:\n1.: Spezifische Kraftwerke der verschiedenen fossilen Energieträger und der Einsatz erneuerbarer Energien sind entsprechend der länderspezifischen Energieträgermixe modelliert. Die Analyse bezieht Stromimporte aus den Nachbarländern, Transmissions-und Verteilungsverluste und den Eigenverbrauch im Kraftwerk und bei der Verteilung bzw. Speicherung, z. B. durch Pumpspeicherwerke, ein.\n2.: Die landes-/regionalspezifischen Technologiestandards sowie die Erzeugung in Elektrizitätskraftwerken und/oder in speziellen Kraftwerken mit Kraft-Wärme-Kopplung (KWK) sind berücksichtigt. \n3.: Die länderspezifische Energieträgerbereitstellung (mit Anteil der Importe und/oder Eigenversorgung) einschließlich der Energieträger-Eigenschaften (z. B. Elementar- und Energiegehalte) werden berücksichtigt. \n4.: Die Förderung, Produktion, Verarbeitung und Transportprozesse werden entsprechend der Situation im jeweiligen Stromerzeugerland modelliert. Die unterschiedlichen Produktions- und Verarbeitungsverfahren (Emissionen und Wirkungsgrade) in den verschiedenen Energieerzeugerländern werden einbezogen, z. B. Rohöl-Veredelungsverfahren oder Abfackel-Raten an den Ölplattformen.\nThermische Energie, Prozessdampf: Die Erzeugung von Dampf und thermischer Energie in Heizkraftwerken wird entsprechend der landesspezifischen Situation (Emissionsgrenzwerte, Energieträgerbasis) modelliert.\nDer Wirkungsgrad für die thermische Energieerzeugung beträgt per Definition 100% des Energieträgereinsatzes. Für Prozessdampf liegt der Wirkungsgrad im Bereich von 85-95%. Die zur Heizenergie-Erzeugung verwendeten Energieträger werden entsprechend der nationalen Situation modelliert (siehe Kapitel Strom oben).\nTransporte: Alle relevanten und bekannten Transportprozesse in Form von See- und Binnenschiffsverkehr sowie Bahn-, Lkw- und der Leitungstransport sind enthalten.\nEnergieträger: Die Energieträger werden entsprechend der spezifischen Versorgungslage modelliert (siehe Kapitel Strom oben). \nRaffinerieprodukte: Diesel, Benzin, technische Gase, Heizöl, Schmierstoffe und Rückstände, wie Bitumen, werden mit einem parametrierten länderspezifische Raffineriemodell modelliert. Das Raffinerie-Modell bezieht die länderspezifischen Veredelungsverfahren (z. B. Emissionspegel, interner Energieverbrauch etc.) und das länderspezifische Produktspektrum ein, das sich je nach Land stark unterscheiden kann. Die Rohöl-Förderung wird gemäß der länderspezifischen Situation mit den jeweiligen Energieträger-Eigenschaften modelliert.", "lang": "de"}], "technologicalApplicability": [{"value": "This product can be used in construction.", "lang": "en"}, {"value": "Dieses Produkt kann im Baubereich verwendet werden.", "lang": "de"}], "referenceToTechnologyPictogramme": {"shortDescription": [{"value": "metals_glo_carbon steel production - bf route.jpg", "lang": "en"}], "type": "source data set", "refObjectId": "c1ee0a75-9fa7-40a9-b4a3-5743cd425842", "version": "24.01.000", "uri": "../sources/c1ee0a75-9fa7-40a9-b4a3-5743cd425842.xml"}, "referenceToTechnologyFlowDiagrammOrPicture": [{"shortDescription": [{"value": "abmessungen stahlrohre.jpg", "lang": "en"}], "type": "source data set", "refObjectId": "2eb8846f-21b3-4c03-b31c-50b4ae01909c", "version": "24.01.000", "uri": "../sources/2eb8846f-21b3-4c03-b31c-50b4ae01909c.xml"}]}}, "modellingAndValidation": {"LCIMethodAndAllocation": {"typeOfDataSet": "EPD", "other": {"anies": [{"name": "subType", "value": "generic dataset"}]}}, "dataSourcesTreatmentAndRepresentativeness": {"referenceToDataSource": [{"shortDescription": [{"value": "VDI 2067", "lang": "en"}], "type": "source data set", "refObjectId": "fe5b9b2f-38c9-430a-b331-c7e9d70fca9d", "version": "24.01.000", "uri": "../sources/fe5b9b2f-38c9-430a-b331-c7e9d70fca9d.xml"}, {"shortDescription": [{"value": "EC 2001", "lang": "en"}], "type": "source data set", "refObjectId": "a20a710e-8582-4659-9cf7-ecb3a5d730dc", "version": "24.01.000", "uri": "../sources/a20a710e-8582-4659-9cf7-ecb3a5d730dc.xml"}, {"shortDescription": [{"value": "BRENSING 1995", "lang": "en"}], "type": "source data set", "refObjectId": "b2cff430-2230-45b2-b005-93f153c6575c", "version": "24.01.000", "uri": "../sources/b2cff430-2230-45b2-b005-93f153c6575c.xml"}, {"shortDescription": [{"value": "DICKINSON 2008", "lang": "en"}], "type": "source data set", "refObjectId": "df10eab3-9c72-40c7-92f0-d123ffa3e51c", "version": "24.01.000", "uri": "../sources/df10eab3-9c72-40c7-92f0-d123ffa3e51c.xml"}, {"shortDescription": [{"value": "Documentation of data quality management", "lang": "en"}], "type": "source data set", "refObjectId": "e3bd9bbf-2c3c-42aa-8892-fd13f1065ca5", "version": "24.01.000", "uri": "../sources/e3bd9bbf-2c3c-42aa-8892-fd13f1065ca5.xml"}, {"shortDescription": [{"value": "GaBi Database Edition 2021, CUP2021.01", "lang": "en"}], "type": "source data set", "refObjectId": "1cece811-7501-44d4-8067-9259bd5cb835", "version": "00.01.000", "uri": "../sources/1cece811-7501-44d4-8067-9259bd5cb835.xml"}, {"shortDescription": [{"value": "Sphera Managed LCA Content Databases (all versions)", "lang": "en"}], "type": "source data set", "refObjectId": "28d74cc0-db8b-4d7e-bc44-5f6d56ce0c4a", "version": "00.03.002", "uri": "../sources/28d74cc0-db8b-4d7e-bc44-5f6d56ce0c4a.xml"}], "useAdviceForDataSet": [{"value": "The data set represents a cradle to gate inventory. It can be used to characterise the supply chain situation of the respective commodity in a representative manner. Combination with individual unit processes using this commodity enables the generation of user-specific (product) LCAs.", "lang": "en"}, {"value": "Der Datensatz repräsentiert ein Cradle to Gate Inventar. Er kann verwendet werden, um die Lieferkette des jeweiligen Produktes in einer repräsentativen Weise zu charakterisieren. Die Kombination mit einzelnen Einheitenprozessen und diesem Produkt ermöglicht die Erstellung von anwenderspezifischen (Produkt-) LCAs.", "lang": "de"}]}, "validation": {"review": [{"referenceToNameOfReviewerAndInstitution": [{"shortDescription": [{"value": "Sphera Solutions GmbH", "lang": "en"}], "type": "contact data set", "refObjectId": "d7fa0337-f279-430d-becf-7f3111a85010", "version": "24.01.000", "uri": "../contacts/d7fa0337-f279-430d-becf-7f3111a85010.xml"}], "type": "Dependent internal review"}, {"referenceToNameOfReviewerAndInstitution": [{"shortDescription": [{"value": "Sphera Product Sustainability user forum", "lang": "en"}], "type": "contact data set", "refObjectId": "8f1306f0-7b83-4f36-a537-aa83f0498266", "version": "24.01.000", "uri": "../contacts/8f1306f0-7b83-4f36-a537-aa83f0498266.xml"}], "type": "Independent external review"}]}, "complianceDeclarations": {"compliance": [{"referenceToComplianceSystem": {"shortDescription": [{"value": "EN 15804+A2 (EF 3.1)", "lang": "de"}, {"value": "EN 15804+A2 (EF 3.1)", "lang": "en"}], "type": "source data set", "refObjectId": "d4aa3ec7-b1d7-4a4a-a6cb-37af88dcc902", "version": "00.01.000", "uri": "../sources/d4aa3ec7-b1d7-4a4a-a6cb-37af88dcc902.xml"}, "approvalOfOverallCompliance": "Fully compliant"}]}}, "administrativeInformation": {"dataGenerator": {"referenceToPersonOrEntityGeneratingTheDataSet": [{"shortDescription": [{"value": "Sphera Solutions GmbH", "lang": "en"}], "type": "contact data set", "refObjectId": "d7fa0337-f279-430d-becf-7f3111a85010", "version": "24.01.000", "uri": "../contacts/d7fa0337-f279-430d-becf-7f3111a85010.xml"}]}, "dataEntryBy": {"timeStamp": 1718121639000, "referenceToDataSetFormat": [{"shortDescription": [{"value": "ILCD format 1.1", "lang": "de"}, {"value": "ILCD format 1.1", "lang": "en"}], "type": "source data set", "refObjectId": "a97a0155-0234-4b87-b4ce-a45da52f2a40", "version": "01.00.000", "uri": "../sources/a97a0155-0234-4b87-b4ce-a45da52f2a40.xml"}, {"shortDescription": [{"value": "EPD-Datenformaterweiterungen v1.2", "lang": "de"}, {"value": "EPD Data Format Extensions v1.2", "lang": "en"}], "type": "source data set", "refObjectId": "a29449fd-aa2f-4de8-b5d7-4b06b43c6fde", "version": "00.01.000", "uri": "../sources/a29449fd-aa2f-4de8-b5d7-4b06b43c6fde.xml"}], "referenceToPersonOrEntityEnteringTheData": {"shortDescription": [{"value": "Sphera Solutions GmbH", "lang": "en"}], "type": "contact data set", "refObjectId": "d7fa0337-f279-430d-becf-7f3111a85010", "version": "24.01.000", "uri": "../contacts/d7fa0337-f279-430d-becf-7f3111a85010.xml"}}, "publicationAndOwnership": {"dataSetVersion": "20.24.070", "referenceToPrecedingDataSetVersion": [{"shortDescription": [{"value": "Steel pipe", "lang": "en"}], "type": "process data set", "refObjectId": "eeda9e75-727c-474d-8c54-3982cafe07d7", "uri": "https://www.oekobaudat.de/OEKOBAU.DAT/resource/processes/eeda9e75-727c-474d-8c54-3982cafe07d7?version=20.23.050"}], "referenceToRegistrationAuthority": {"shortDescription": [{"value": "Sphera Solutions GmbH", "lang": "en"}], "type": "contact data set", "refObjectId": "d7fa0337-f279-430d-becf-7f3111a85010", "version": "24.01.000", "uri": "../contacts/d7fa0337-f279-430d-becf-7f3111a85010.xml"}, "referenceToOwnershipOfDataSet": {"shortDescription": [{"value": "Sphera Solutions GmbH", "lang": "en"}], "type": "contact data set", "refObjectId": "d7fa0337-f279-430d-becf-7f3111a85010", "version": "24.01.000", "uri": "../contacts/d7fa0337-f279-430d-becf-7f3111a85010.xml"}, "copyright": true, "licenseType": "Free of charge for all users and uses", "accessRestrictions": [{"value": "The license conditions as stated on https://www.oekobaudat.de/apply.", "lang": "en"}, {"value": "Es gelten die Lizenzbedingungen wie sie auf https://www.oekobaudat.de/ genannt sind.", "lang": "de"}], "other": {"anies": [{"name": "referenceToPublisher", "value": {"shortDescription": [{"value": "BBSR", "lang": "en"}], "type": "contact data set", "refObjectId": "f11651e0-7877-11e3-981f-0800200c9a66", "version": "00.01.000", "uri": "../contacts/f11651e0-7877-11e3-981f-0800200c9a66.xml"}}]}}}, "exchanges": {"exchange": [{"dataSetInternalID": 101140, "referenceToFlowDataSet": {"shortDescription": [{"value": "Steel pipe", "lang": "en"}, {"value": "Stahlrohr", "lang": "de"}], "type": "flow data set", "refObjectId": "9eeecef3-a893-477b-a8e1-6f7480233f30", "version": "24.01.000", "uri": "../flows/9eeecef3-a893-477b-a8e1-6f7480233f30.xml"}, "meanAmount": 1.0, "referenceFlow": true, "resultingflowAmount": 1.0, "flowProperties": [{"name": [{"lang": "en", "value": "Mass"}, {"lang": "de", "value": "Masse"}], "uuid": "93a60a56-a3c8-11da-a746-0800200b9a66", "referenceFlowProperty": true, "meanValue": 1.0, "referenceUnit": "kg", "unitGroupUUID": "ad38d542-3fe9-439d-9b95-2f5f7752acaf"}], "materialProperties": [{"name": "gross density", "value": "7850.0", "unit": "kg/m^3", "unitDescription": "kilograms per cubic metre"}], "typeOfFlow": "Product flow", "classification": {"classHierarchy": "Valuable substances / Materials / Metals", "name": "GaBiCategories"}}, {"dataSetInternalID": 101141, "referenceToFlowDataSet": {"shortDescription": [{"value": "Use of renewable primary energy as energy carrier (PERE)", "lang": "en"}, {"value": "Erneuerbare Primärenergie als Energieträger (PERE)", "lang": "de"}], "type": "flow data set", "refObjectId": "20f32be5-0398-4288-9b6d-accddd195317", "version": "24.01.000", "uri": "../flows/20f32be5-0398-4288-9b6d-accddd195317.xml"}, "exchange direction": "INPUT", "other": {"anies": [{"value": "2.41094570110095", "module": "A1-A3"}, {"name": "referenceToUnitGroupDataSet", "value": {"shortDescription": [{"value": "MJ", "lang": "en"}], "type": "unit group data set", "refObjectId": "93a60a57-a3c8-11da-a746-0800200c9a66", "version": "03.00.000", "uri": "../unitgroups/93a60a57-a3c8-11da-a746-0800200c9a66.xml"}}, {"value": "0.0472140331287191", "module": "C2"}, {"value": "0", "module": "C3"}, {"value": "0.00380115010733422", "module": "C4"}, {"value": "2.12896379128461", "module": "D"}]}, "resolvedFlowVersion": "38.00.000", "flowProperties": [], "typeOfFlow": "Other flow", "classification": {"classHierarchy": "Quantities", "name": "GaBiCategories"}}, {"dataSetInternalID": 101142, "referenceToFlowDataSet": {"shortDescription": [{"value": "Use of renewable primary energy resources used as raw materials (PERM)", "lang": "en"}, {"value": "Erneuerbare Primärenergie zur stofflichen Nutzung (PERM)", "lang": "de"}], "type": "flow data set", "refObjectId": "fb3ec0de-548d-4508-aea5-00b73bf6f702", "version": "24.01.000", "uri": "../flows/fb3ec0de-548d-4508-aea5-00b73bf6f702.xml"}, "exchange direction": "INPUT", "other": {"anies": [{"value": "0", "module": "A1-A3"}, {"name": "referenceToUnitGroupDataSet", "value": {"shortDescription": [{"value": "MJ", "lang": "en"}], "type": "unit group data set", "refObjectId": "93a60a57-a3c8-11da-a746-0800200c9a66", "version": "03.00.000", "uri": "../unitgroups/93a60a57-a3c8-11da-a746-0800200c9a66.xml"}}, {"value": "0", "module": "C2"}, {"value": "0", "module": "C3"}, {"value": "0", "module": "C4"}, {"value": "0", "module": "D"}]}, "resolvedFlowVersion": "38.00.000", "flowProperties": [], "typeOfFlow": "Other flow", "classification": {"classHierarchy": "Quantities", "name": "GaBiCategories"}}, {"dataSetInternalID": 101143, "referenceToFlowDataSet": {"shortDescription": [{"value": "Total use of renewable primary energy (PERT)", "lang": "en"}, {"value": "Total erneuerbare Primärenergie (PERT)", "lang": "de"}], "type": "flow data set", "refObjectId": "53f97275-fa8a-4cdd-9024-65936002acd0", "version": "24.01.000", "uri": "../flows/53f97275-fa8a-4cdd-9024-65936002acd0.xml"}, "exchange direction": "INPUT", "other": {"anies": [{"value": "2.41094570110095", "module": "A1-A3"}, {"name": "referenceToUnitGroupDataSet", "value": {"shortDescription": [{"value": "MJ", "lang": "en"}], "type": "unit group data set", "refObjectId": "93a60a57-a3c8-11da-a746-0800200c9a66", "version": "03.00.000", "uri": "../unitgroups/93a60a57-a3c8-11da-a746-0800200c9a66.xml"}}, {"value": "0.0472140331287191", "module": "C2"}, {"value": "0", "module": "C3"}, {"value": "0.00380115010733422", "module": "C4"}, {"value": "2.12896379128461", "module": "D"}]}, "resolvedFlowVersion": "38.00.000", "flowProperties": [], "typeOfFlow": "Other flow", "classification": {"classHierarchy": "Quantities / Environmental quantities / EPD EN 15804 / LCI indicators", "name": "GaBiCategories"}}, {"dataSetInternalID": 101144, "referenceToFlowDataSet": {"shortDescription": [{"value": "Use of non renewable primary energy as energy carrier (PENRE)", "lang": "en"}, {"value": "Nicht-erneuerbare Primärenergie als Energieträger (PENRE)", "lang": "de"}], "type": "flow data set", "refObjectId": "ac857178-2b45-46ec-892a-a9a4332f0372", "version": "24.01.000", "uri": "../flows/ac857178-2b45-46ec-892a-a9a4332f0372.xml"}, "exchange direction": "INPUT", "other": {"anies": [{"value": "22.7593479964009", "module": "A1-A3"}, {"name": "referenceToUnitGroupDataSet", "value": {"shortDescription": [{"value": "MJ", "lang": "en"}], "type": "unit group data set", "refObjectId": "93a60a57-a3c8-11da-a746-0800200c9a66", "version": "03.00.000", "uri": "../unitgroups/93a60a57-a3c8-11da-a746-0800200c9a66.xml"}}, {"value": "0.126744694324671", "module": "C2"}, {"value": "0", "module": "C3"}, {"value": "0.0217080114977854", "module": "C4"}, {"value": "-10.0892924877623", "module": "D"}]}, "resolvedFlowVersion": "38.00.000", "flowProperties": [], "typeOfFlow": "Other flow", "classification": {"classHierarchy": "Quantities", "name": "GaBiCategories"}}, {"dataSetInternalID": 101145, "referenceToFlowDataSet": {"shortDescription": [{"value": "Use of non renewable primary energy resources used as raw materials (PENRM)", "lang": "en"}, {"value": "Nicht-erneuerbare Primärenergie zur stofflichen Nutzung (PENRM)", "lang": "de"}], "type": "flow data set", "refObjectId": "1421caa0-679d-4bf4-b282-0eb850ccae27", "version": "24.01.000", "uri": "../flows/1421caa0-679d-4bf4-b282-0eb850ccae27.xml"}, "exchange direction": "INPUT", "other": {"anies": [{"value": "0", "module": "A1-A3"}, {"name": "referenceToUnitGroupDataSet", "value": {"shortDescription": [{"value": "MJ", "lang": "en"}], "type": "unit group data set", "refObjectId": "93a60a57-a3c8-11da-a746-0800200c9a66", "version": "03.00.000", "uri": "../unitgroups/93a60a57-a3c8-11da-a746-0800200c9a66.xml"}}, {"value": "0", "module": "C2"}, {"value": "0", "module": "C3"}, {"value": "0", "module": "C4"}, {"value": "0", "module": "D"}]}, "resolvedFlowVersion": "38.00.000", "flowProperties": [], "typeOfFlow": "Other flow", "classification": {"classHierarchy": "Quantities", "name": "GaBiCategories"}}, {"dataSetInternalID": 101146, "referenceToFlowDataSet": {"shortDescription": [{"value": "Total use of non renewable primary energy resource (PENRT)", "lang": "en"}, {"value": "Total nicht-erneuerbare Primärenergie (PENRT)", "lang": "de"}], "type": "flow data set", "refObjectId": "06159210-646b-4c8d-8583-da9b3b95a6c1", "version": "24.01.000", "uri": "../flows/06159210-646b-4c8d-8583-da9b3b95a6c1.xml"}, "exchange direction": "INPUT", "other": {"anies": [{"value": "22.7593479964009", "module": "A1-A3"}, {"name": "referenceToUnitGroupDataSet", "value": {"shortDescription": [{"value": "MJ", "lang": "en"}], "type": "unit group data set", "refObjectId": "93a60a57-a3c8-11da-a746-0800200c9a66", "version": "03.00.000", "uri": "../unitgroups/93a60a57-a3c8-11da-a746-0800200c9a66.xml"}}, {"value": "0.126744694324671", "module": "C2"}, {"value": "0", "module": "C3"}, {"value": "0.0217080114977854", "module": "C4"}, {"value": "-10.0892924877623", "module": "D"}]}, "resolvedFlowVersion": "38.00.000", "flowProperties": [], "typeOfFlow": "Other flow", "classification": {"classHierarchy": "Quantities / Environmental quantities / EPD EN 15804 / LCI indicators", "name": "GaBiCategories"}}, {"dataSetInternalID": 101147, "referenceToFlowDataSet": {"shortDescription": [{"value": "Use of secondary material (SM)", "lang": "en"}, {"value": "Einsatz von Sekundärstoffen (SM)", "lang": "de"}], "type": "flow data set", "refObjectId": "c6a1f35f-2d09-4f54-8dfb-97e502e1ce92", "version": "24.01.000", "uri": "../flows/c6a1f35f-2d09-4f54-8dfb-97e502e1ce92.xml"}, "exchange direction": "INPUT", "other": {"anies": [{"value": "0.181927564966266", "module": "A1-A3"}, {"name": "referenceToUnitGroupDataSet", "value": {"shortDescription": [{"value": "kg", "lang": "en"}], "type": "unit group data set", "refObjectId": "93a60a57-a4c8-11da-a746-0800200c9a66", "version": "03.00.000", "uri": "../unitgroups/93a60a57-a4c8-11da-a746-0800200c9a66.xml"}}, {"value": "0", "module": "C2"}, {"value": "0", "module": "C3"}, {"value": "0", "module": "C4"}, {"value": "0", "module": "D"}]}, "resolvedFlowVersion": "38.00.000", "flowProperties": [], "typeOfFlow": "Other flow", "classification": {"classHierarchy": "Quantities / Environmental quantities / EPD EN 15804 / LCI indicators", "name": "GaBiCategories"}}, {"dataSetInternalID": 101148, "referenceToFlowDataSet": {"shortDescription": [{"value": "Use of renewable secondary fuels (SF)", "lang": "en"}, {"value": "Erneuerbare Sekundärbrennstoffe (SF)", "lang": "de"}], "type": "flow data set", "refObjectId": "64333088-a55f-4aa2-9a31-c10b07816787", "version": "24.01.000", "uri": "../flows/64333088-a55f-4aa2-9a31-c10b07816787.xml"}, "exchange direction": "INPUT", "other": {"anies": [{"value": "0", "module": "A1-A3"}, {"name": "referenceToUnitGroupDataSet", "value": {"shortDescription": [{"value": "MJ", "lang": "en"}], "type": "unit group data set", "refObjectId": "93a60a57-a3c8-11da-a746-0800200c9a66", "version": "03.00.000", "uri": "../unitgroups/93a60a57-a3c8-11da-a746-0800200c9a66.xml"}}, {"value": "0", "module": "C2"}, {"value": "0", "module": "C3"}, {"value": "0", "module": "C4"}, {"value": "0", "module": "D"}]}, "resolvedFlowVersion": "38.00.000", "flowProperties": [], "typeOfFlow": "Other flow", "classification": {"classHierarchy": "Quantities / Environmental quantities / EPD EN 15804 / LCI indicators", "name": "GaBiCategories"}}, {"dataSetInternalID": 101149, "referenceToFlowDataSet": {"shortDescription": [{"value": "Use of non renewable secondary fuels (NRSF)", "lang": "en"}, {"value": "Nicht erneuerbare Sekundärbrennstoffe (NRSF)", "lang": "de"}], "type": "flow data set", "refObjectId": "89def144-d39a-4287-b86f-efde453ddcb2", "version": "24.01.000", "uri": "../flows/89def144-d39a-4287-b86f-efde453ddcb2.xml"}, "exchange direction": "INPUT", "other": {"anies": [{"value": "0", "module": "A1-A3"}, {"name": "referenceToUnitGroupDataSet", "value": {"shortDescription": [{"value": "MJ", "lang": "en"}], "type": "unit group data set", "refObjectId": "93a60a57-a3c8-11da-a746-0800200c9a66", "version": "03.00.000", "uri": "../unitgroups/93a60a57-a3c8-11da-a746-0800200c9a66.xml"}}, {"value": "0", "module": "C2"}, {"value": "0", "module": "C3"}, {"value": "0", "module": "C4"}, {"value": "0", "module": "D"}]}, "resolvedFlowVersion": "38.00.000", "flowProperties": [], "typeOfFlow": "Other flow", "classification": {"classHierarchy": "Quantities / Environmental quantities / EPD EN 15804 / LCI indicators", "name": "GaBiCategories"}}, {"dataSetInternalID": 101150, "referenceToFlowDataSet": {"shortDescription": [{"value": "Net use of fresh water (FW)", "lang": "en"}, {"value": "Nettoeinsatz von Süßwasserressourcen (FW)", "lang": "de"}], "type": "flow data set", "refObjectId": "3cf952c8-f3a4-461d-8c96-96456ca62246", "version": "24.01.000", "uri": "../flows/3cf952c8-f3a4-461d-8c96-96456ca62246.xml"}, "exchange direction": "INPUT", "other": {"anies": [{"value": "0.00161012428614406", "module": "A1-A3"}, {"name": "referenceToUnitGroupDataSet", "value": {"shortDescription": [{"value": "m3", "lang": "en"}], "type": "unit group data set", "refObjectId": "93a60a57-a3c8-12da-a746-0800200c9a66", "version": "03.00.000", "uri": "../unitgroups/93a60a57-a3c8-12da-a746-0800200c9a66.xml"}}, {"value": "2.09554350275876E-5", "module": "C2"}, {"value": "0", "module": "C3"}, {"value": "5.74321633565582E-6", "module": "C4"}, {"value": "-0.000890347127013153", "module": "D"}]}, "resolvedFlowVersion": "38.00.000", "flowProperties": [], "typeOfFlow": "Other flow", "classification": {"classHierarchy": "Quantities / Environmental quantities / EPD EN 15804 / LCI indicators", "name": "GaBiCategories"}}, {"dataSetInternalID": 101151, "referenceToFlowDataSet": {"shortDescription": [{"value": "Hazardous waste disposed (HWD)", "lang": "en"}, {"value": "Gefährlicher Abfall zur Deponie (HWD)", "lang": "de"}], "type": "flow data set", "refObjectId": "430f9e0f-59b2-46a0-8e0d-55e0e84948fc", "version": "24.01.000", "uri": "../flows/430f9e0f-59b2-46a0-8e0d-55e0e84948fc.xml"}, "exchange direction": "OUTPUT", "other": {"anies": [{"value": "4.6815616745545E-9", "module": "A1-A3"}, {"name": "referenceToUnitGroupDataSet", "value": {"shortDescription": [{"value": "kg", "lang": "en"}], "type": "unit group data set", "refObjectId": "93a60a57-a4c8-11da-a746-0800200c9a66", "version": "03.00.000", "uri": "../unitgroups/93a60a57-a4c8-11da-a746-0800200c9a66.xml"}}, {"value": "8.20956972641144E-11", "module": "C2"}, {"value": "0", "module": "C3"}, {"value": "5.44787172586401E-12", "module": "C4"}, {"value": "5.43287167050197E-9", "module": "D"}]}, "resolvedFlowVersion": "38.00.000", "flowProperties": [], "typeOfFlow": "Other flow", "classification": {"classHierarchy": "Quantities / Environmental quantities / EPD EN 15804 / LCI indicators", "name": "GaBiCategories"}}, {"dataSetInternalID": 101152, "referenceToFlowDataSet": {"shortDescription": [{"value": "Non harzardous waste disposed (NHWD)", "lang": "en"}, {"value": "Entsorgter nicht gefährlicher Abfall (NHWD)", "lang": "de"}], "type": "flow data set", "refObjectId": "b29ef66b-e286-4afa-949f-62f1a7b4d7fa", "version": "24.01.000", "uri": "../flows/b29ef66b-e286-4afa-949f-62f1a7b4d7fa.xml"}, "exchange direction": "OUTPUT", "other": {"anies": [{"value": "0.0308563007991262", "module": "A1-A3"}, {"name": "referenceToUnitGroupDataSet", "value": {"shortDescription": [{"value": "kg", "lang": "en"}], "type": "unit group data set", "refObjectId": "93a60a57-a4c8-11da-a746-0800200c9a66", "version": "03.00.000", "uri": "../unitgroups/93a60a57-a4c8-11da-a746-0800200c9a66.xml"}}, {"value": "5.03828894451032E-5", "module": "C2"}, {"value": "0", "module": "C3"}, {"value": "0.110105163941318", "module": "C4"}, {"value": "-0.0199162826423479", "module": "D"}]}, "resolvedFlowVersion": "38.00.000", "flowProperties": [], "typeOfFlow": "Other flow", "classification": {"classHierarchy": "Quantities / Environmental quantities / EPD EN 15804 / LCI indicators", "name": "GaBiCategories"}}, {"dataSetInternalID": 101153, "referenceToFlowDataSet": {"shortDescription": [{"value": "Radioactive waste disposed (RWD)", "lang": "en"}, {"value": "Entsorgter radioaktiver Abfall (RWD)", "lang": "de"}], "type": "flow data set", "refObjectId": "3449546e-52ad-4b39-b809-9fb77cea8ff6", "version": "24.01.000", "uri": "../flows/3449546e-52ad-4b39-b809-9fb77cea8ff6.xml"}, "exchange direction": "OUTPUT", "other": {"anies": [{"value": "0.00017705030145446", "module": "A1-A3"}, {"name": "referenceToUnitGroupDataSet", "value": {"shortDescription": [{"value": "kg", "lang": "en"}], "type": "unit group data set", "refObjectId": "93a60a57-a4c8-11da-a746-0800200c9a66", "version": "03.00.000", "uri": "../unitgroups/93a60a57-a4c8-11da-a746-0800200c9a66.xml"}}, {"value": "2.12513181137391E-6", "module": "C2"}, {"value": "0", "module": "C3"}, {"value": "2.24587725011341E-7", "module": "C4"}, {"value": "0.000192766442772254", "module": "D"}]}, "resolvedFlowVersion": "38.00.000", "flowProperties": [], "typeOfFlow": "Other flow", "classification": {"classHierarchy": "Quantities / Environmental quantities / EPD EN 15804 / LCI indicators", "name": "GaBiCategories"}}, {"dataSetInternalID": 101154, "referenceToFlowDataSet": {"shortDescription": [{"value": "Components for re-use (CRU)", "lang": "en"}, {"value": "Komponenten für die Wiederverwendung (CRU)", "lang": "de"}], "type": "flow data set", "refObjectId": "a2b32f97-3fc7-4af2-b209-525bc6426f33", "version": "24.01.000", "uri": "../flows/a2b32f97-3fc7-4af2-b209-525bc6426f33.xml"}, "exchange direction": "OUTPUT", "other": {"anies": [{"value": "0", "module": "A1-A3"}, {"name": "referenceToUnitGroupDataSet", "value": {"shortDescription": [{"value": "kg", "lang": "en"}], "type": "unit group data set", "refObjectId": "93a60a57-a4c8-11da-a746-0800200c9a66", "version": "03.00.000", "uri": "../unitgroups/93a60a57-a4c8-11da-a746-0800200c9a66.xml"}}, {"value": "0", "module": "C2"}, {"value": "0", "module": "C3"}, {"value": "0", "module": "C4"}, {"value": "0", "module": "D"}]}, "resolvedFlowVersion": "38.00.000", "flowProperties": [], "typeOfFlow": "Other flow", "classification": {"classHierarchy": "Quantities / Environmental quantities / EPD EN 15804 / LCI indicators", "name": "GaBiCategories"}}, {"dataSetInternalID": 101155, "referenceToFlowDataSet": {"shortDescription": [{"value": "Materials for recycling  (MFR)", "lang": "en"}, {"value": "Stoffe zum Recycling (MFR)", "lang": "de"}], "type": "flow data set", "refObjectId": "d7fe48a5-4103-49c8-9aae-b0b5dfdbd6ae", "version": "24.01.000", "uri": "../flows/d7fe48a5-4103-49c8-9aae-b0b5dfdbd6ae.xml"}, "exchange direction": "OUTPUT", "other": {"anies": [{"value": "0", "module": "A1-A3"}, {"name": "referenceToUnitGroupDataSet", "value": {"shortDescription": [{"value": "kg", "lang": "en"}], "type": "unit group data set", "refObjectId": "93a60a57-a4c8-11da-a746-0800200c9a66", "version": "03.00.000", "uri": "../unitgroups/93a60a57-a4c8-11da-a746-0800200c9a66.xml"}}, {"value": "0", "module": "C2"}, {"value": "0.9", "module": "C3"}, {"value": "0", "module": "C4"}, {"value": "0", "module": "D"}]}, "resolvedFlowVersion": "38.00.000", "flowProperties": [], "typeOfFlow": "Other flow", "classification": {"classHierarchy": "Quantities / Environmental quantities / EPD EN 15804 / LCI indicators", "name": "GaBiCategories"}}, {"dataSetInternalID": 101156, "referenceToFlowDataSet": {"shortDescription": [{"value": "Materials for energy recovery (MER)", "lang": "en"}, {"value": "Stoffe für die Energierückgewinnung (MER)", "lang": "de"}], "type": "flow data set", "refObjectId": "59a9181c-3aaf-46ee-8b13-2b3723b6e447", "version": "24.01.000", "uri": "../flows/59a9181c-3aaf-46ee-8b13-2b3723b6e447.xml"}, "exchange direction": "OUTPUT", "other": {"anies": [{"value": "0", "module": "A1-A3"}, {"name": "referenceToUnitGroupDataSet", "value": {"shortDescription": [{"value": "kg", "lang": "en"}], "type": "unit group data set", "refObjectId": "93a60a57-a4c8-11da-a746-0800200c9a66", "version": "03.00.000", "uri": "../unitgroups/93a60a57-a4c8-11da-a746-0800200c9a66.xml"}}, {"value": "0", "module": "C2"}, {"value": "0", "module": "C3"}, {"value": "0", "module": "C4"}, {"value": "0", "module": "D"}]}, "resolvedFlowVersion": "38.00.000", "flowProperties": [], "typeOfFlow": "Other flow", "classification": {"classHierarchy": "Quantities / Environmental quantities / EPD EN 15804 / LCI indicators", "name": "GaBiCategories"}}, {"dataSetInternalID": 101157, "referenceToFlowDataSet": {"shortDescription": [{"value": "Exported electrical energy (EEE)", "lang": "en"}, {"value": "Exportierte elektrische Energie (EEE)", "lang": "de"}], "type": "flow data set", "refObjectId": "4da0c987-2b76-40d6-9e9e-82a017aaaf29", "version": "24.01.000", "uri": "../flows/4da0c987-2b76-40d6-9e9e-82a017aaaf29.xml"}, "exchange direction": "OUTPUT", "other": {"anies": [{"value": "0", "module": "A1-A3"}, {"name": "referenceToUnitGroupDataSet", "value": {"shortDescription": [{"value": "MJ", "lang": "en"}], "type": "unit group data set", "refObjectId": "93a60a57-a3c8-11da-a746-0800200c9a66", "version": "03.00.000", "uri": "../unitgroups/93a60a57-a3c8-11da-a746-0800200c9a66.xml"}}, {"value": "0", "module": "C2"}, {"value": "0", "module": "C3"}, {"value": "0", "module": "C4"}, {"value": "0", "module": "D"}]}, "resolvedFlowVersion": "38.00.000", "flowProperties": [], "typeOfFlow": "Other flow", "classification": {"classHierarchy": "Quantities / Environmental quantities / EPD EN 15804 / LCI indicators", "name": "GaBiCategories"}}, {"dataSetInternalID": 101158, "referenceToFlowDataSet": {"shortDescription": [{"value": "Exported thermal energy (EET)", "lang": "en"}, {"value": "Exportierte thermische Energie (EET)", "lang": "de"}], "type": "flow data set", "refObjectId": "98daf38a-7a79-46d3-9a37-2b7bd0955810", "version": "24.01.000", "uri": "../flows/98daf38a-7a79-46d3-9a37-2b7bd0955810.xml"}, "exchange direction": "OUTPUT", "other": {"anies": [{"value": "0", "module": "A1-A3"}, {"name": "referenceToUnitGroupDataSet", "value": {"shortDescription": [{"value": "MJ", "lang": "en"}], "type": "unit group data set", "refObjectId": "93a60a57-a3c8-11da-a746-0800200c9a66", "version": "03.00.000", "uri": "../unitgroups/93a60a57-a3c8-11da-a746-0800200c9a66.xml"}}, {"value": "0", "module": "C2"}, {"value": "0", "module": "C3"}, {"value": "0", "module": "C4"}, {"value": "0", "module": "D"}]}, "resolvedFlowVersion": "38.00.000", "flowProperties": [], "typeOfFlow": "Other flow", "classification": {"classHierarchy": "Quantities / Environmental quantities / EPD EN 15804 / LCI indicators", "name": "GaBiCategories"}}]}, "LCIAResults": {"LCIAResult": [{"referenceToLCIAMethodDataSet": {"shortDescription": [{"value": "Climate change", "lang": "en"}, {"value": "Globales Erwärmungspotenzial - total (GWP-total)", "lang": "de"}], "type": "LCIA method data set", "refObjectId": "a7ea142a-9749-11ed-a8fc-0242ac120002", "version": "24.01.000", "uri": "../lciamethods/a7ea142a-9749-11ed-a8fc-0242ac120002.xml"}, "other": {"anies": [{"value": "2.49119095715841", "module": "A1-A3"}, {"value": "0.0100772533213305", "module": "C2"}, {"value": "0", "module": "C3"}, {"value": "0.00164686494353777", "module": "C4"}, {"value": "-1.32349983793772", "module": "D"}, {"name": "referenceToUnitGroupDataSet", "value": {"shortDescription": [{"value": "kg CO2 eq.", "lang": "en"}], "type": "unit group data set", "refObjectId": "1ebf3012-d0db-4de2-aefd-ef30cedb0be1", "version": "25.00.000", "uri": "../unitgroups/1ebf3012-d0db-4de2-aefd-ef30cedb0be1.xml"}}]}}, {"referenceToLCIAMethodDataSet": {"shortDescription": [{"value": "Climate change-Fossil", "lang": "en"}, {"value": "Globales Erwärmungspotenzial - fossil (GWP-fossil)", "lang": "de"}], "type": "LCIA method data set", "refObjectId": "a7ea19c0-9749-11ed-a8fc-0242ac120002", "version": "24.01.000", "uri": "../lciamethods/a7ea19c0-9749-11ed-a8fc-0242ac120002.xml"}, "other": {"anies": [{"value": "2.4885786590198", "module": "A1-A3"}, {"value": "0.0101029439455919", "module": "C2"}, {"value": "0", "module": "C3"}, {"value": "0.00164726895533837", "module": "C4"}, {"value": "-1.32520955653238", "module": "D"}, {"name": "referenceToUnitGroupDataSet", "value": {"shortDescription": [{"value": "kg CO2 eq.", "lang": "en"}], "type": "unit group data set", "refObjectId": "1ebf3012-d0db-4de2-aefd-ef30cedb0be1", "version": "25.00.000", "uri": "../unitgroups/1ebf3012-d0db-4de2-aefd-ef30cedb0be1.xml"}}]}}, {"referenceToLCIAMethodDataSet": {"shortDescription": [{"value": "Climate change-Biogenic", "lang": "en"}, {"value": "Globales Erwärmungspotenzial - biogen (GWP-biogenic)", "lang": "de"}], "type": "LCIA method data set", "refObjectId": "a7ea186c-9749-11ed-a8fc-0242ac120002", "version": "24.01.000", "uri": "../lciamethods/a7ea186c-9749-11ed-a8fc-0242ac120002.xml"}, "other": {"anies": [{"value": "0.00141582088012433", "module": "A1-A3"}, {"value": "-0.000166056147395669", "module": "C2"}, {"value": "0", "module": "C3"}, {"value": "-1.02842976775634E-5", "module": "C4"}, {"value": "0.00235696434050456", "module": "D"}, {"name": "referenceToUnitGroupDataSet", "value": {"shortDescription": [{"value": "kg CO2 eq.", "lang": "en"}], "type": "unit group data set", "refObjectId": "1ebf3012-d0db-4de2-aefd-ef30cedb0be1", "version": "25.00.000", "uri": "../unitgroups/1ebf3012-d0db-4de2-aefd-ef30cedb0be1.xml"}}]}}, {"referenceToLCIAMethodDataSet": {"shortDescription": [{"value": "Climate change-Land use and land use change", "lang": "en"}, {"value": "Globales Erwärmungspotenzial - luluc (GWP-luluc)", "lang": "de"}], "type": "LCIA method data set", "refObjectId": "a7ea1ae2-9749-11ed-a8fc-0242ac120002", "version": "24.01.000", "uri": "../lciamethods/a7ea1ae2-9749-11ed-a8fc-0242ac120002.xml"}, "other": {"anies": [{"value": "0.00119647725848825", "module": "A1-A3"}, {"value": "0.000140365523134253", "module": "C2"}, {"value": "0", "module": "C3"}, {"value": "9.88028587696156E-6", "module": "C4"}, {"value": "-0.000647245745842496", "module": "D"}, {"name": "referenceToUnitGroupDataSet", "value": {"shortDescription": [{"value": "kg CO2 eq.", "lang": "en"}], "type": "unit group data set", "refObjectId": "1ebf3012-d0db-4de2-aefd-ef30cedb0be1", "version": "25.00.000", "uri": "../unitgroups/1ebf3012-d0db-4de2-aefd-ef30cedb0be1.xml"}}]}}, {"referenceToLCIAMethodDataSet": {"shortDescription": [{"value": "Depletion potenzial of the stratospheric ozone layer (ODP)", "lang": "en"}, {"value": "Abbaupotenzial der stratosphärischen Ozonschicht (ODP)", "lang": "de"}], "type": "LCIA method data set", "refObjectId": "b5c629d6-def3-11e6-bf01-fe55135034f3", "version": "24.01.000", "uri": "../lciamethods/b5c629d6-def3-11e6-bf01-fe55135034f3.xml"}, "other": {"anies": [{"value": "4.59854035220188E-12", "module": "A1-A3"}, {"value": "9.27897911101364E-14", "module": "C2"}, {"value": "0", "module": "C3"}, {"value": "4.48817544084644E-15", "module": "C4"}, {"value": "5.0583554206903E-12", "module": "D"}, {"name": "referenceToUnitGroupDataSet", "value": {"shortDescription": [{"value": "kg CFC-11 eq.", "lang": "en"}], "type": "unit group data set", "refObjectId": "d9e957c9-7309-4474-bf3a-7777df6c4e5b", "version": "25.00.000", "uri": "../unitgroups/d9e957c9-7309-4474-bf3a-7777df6c4e5b.xml"}}]}}, {"referenceToLCIAMethodDataSet": {"shortDescription": [{"value": "Acidifcation potential, Accumulated Exceedance (AP)", "lang": "en"}, {"value": "Versauerungspotenzial, kumulierte Überschreitung (AP)", "lang": "de"}], "type": "LCIA method data set", "refObjectId": "b5c611c6-def3-11e6-bf01-fe55135034f3", "version": "24.01.000", "uri": "../lciamethods/b5c611c6-def3-11e6-bf01-fe55135034f3.xml"}, "other": {"anies": [{"value": "0.00552899973885145", "module": "A1-A3"}, {"value": "6.51285645304831E-5", "module": "C2"}, {"value": "0", "module": "C3"}, {"value": "1.16915102494174E-5", "module": "C4"}, {"value": "-0.00303765206457467", "module": "D"}, {"name": "referenceToUnitGroupDataSet", "value": {"shortDescription": [{"value": "Mole of H+ eq.", "lang": "en"}], "type": "unit group data set", "refObjectId": "42e089ac-92bf-4bf2-8ca1-5fc40d18f2ed", "version": "00.01.000", "uri": "../unitgroups/42e089ac-92bf-4bf2-8ca1-5fc40d18f2ed.xml"}}]}}, {"referenceToLCIAMethodDataSet": {"shortDescription": [{"value": "Eutrophication, freshwater", "lang": "en"}, {"value": "Eutrophierungspotenzial - Süßwasser (EP-freshwater)", "lang": "de"}], "type": "LCIA method data set", "refObjectId": "b53ec18f-7377-4ad3-86eb-cc3f4f276b2b", "version": "24.01.000", "uri": "../lciamethods/b53ec18f-7377-4ad3-86eb-cc3f4f276b2b.xml"}, "other": {"anies": [{"value": "2.30187345133413E-6", "module": "A1-A3"}, {"value": "3.41475359118308E-8", "module": "C2"}, {"value": "0", "module": "C3"}, {"value": "3.75261609559579E-9", "module": "C4"}, {"value": "-1.26495479765142E-7", "module": "D"}, {"name": "referenceToUnitGroupDataSet", "value": {"shortDescription": [{"value": "kg P eq.", "lang": "en"}], "type": "unit group data set", "refObjectId": "0429039d-a61d-4590-ba67-aa4a20a810a1", "version": "25.00.000", "uri": "../unitgroups/0429039d-a61d-4590-ba67-aa4a20a810a1.xml"}}]}}, {"referenceToLCIAMethodDataSet": {"shortDescription": [{"value": "Eutrophication marine", "lang": "en"}, {"value": "Eutrophierungspotenzial - Salzwasser (EP-marine)", "lang": "de"}], "type": "LCIA method data set", "refObjectId": "b5c619fa-def3-11e6-bf01-fe55135034f3", "version": "24.01.000", "uri": "../lciamethods/b5c619fa-def3-11e6-bf01-fe55135034f3.xml"}, "other": {"anies": [{"value": "0.00144247994284174", "module": "A1-A3"}, {"value": "3.18002352618182E-5", "module": "C2"}, {"value": "0", "module": "C3"}, {"value": "3.00996661371055E-6", "module": "C4"}, {"value": "-0.000737757354781534", "module": "D"}, {"name": "referenceToUnitGroupDataSet", "value": {"shortDescription": [{"value": "kg N eq.", "lang": "en"}], "type": "unit group data set", "refObjectId": "d05bb823-ecdf-4686-8c40-bf1d9257859f", "version": "00.00.003", "uri": "../unitgroups/d05bb823-ecdf-4686-8c40-bf1d9257859f.xml"}}]}}, {"referenceToLCIAMethodDataSet": {"shortDescription": [{"value": "Eutrophication, terrestrial", "lang": "en"}, {"value": "Eutrophierungspotenzial - Land (EP-terrestrial)", "lang": "de"}], "type": "LCIA method data set", "refObjectId": "b5c614d2-def3-11e6-bf01-fe55135034f3", "version": "24.01.000", "uri": "../lciamethods/b5c614d2-def3-11e6-bf01-fe55135034f3.xml"}, "other": {"anies": [{"value": "0.0155589723246021", "module": "A1-A3"}, {"value": "0.000351084769899465", "module": "C2"}, {"value": "0", "module": "C3"}, {"value": "3.31444961582344E-5", "module": "C4"}, {"value": "-0.00798929892118432", "module": "D"}, {"name": "referenceToUnitGroupDataSet", "value": {"shortDescription": [{"value": "Mole of N eq.", "lang": "en"}], "type": "unit group data set", "refObjectId": "71b4d617-0ec9-4d3f-b65e-e438940c2401", "version": "00.00.003", "uri": "../unitgroups/71b4d617-0ec9-4d3f-b65e-e438940c2401.xml"}}]}}, {"referenceToLCIAMethodDataSet": {"shortDescription": [{"value": "Photochemical Ozone Creation Potential  (POCP)", "lang": "en"}, {"value": "Bildungspotenzial für troposphärisches Ozon (POCP)", "lang": "de"}], "type": "LCIA method data set", "refObjectId": "b5c610fe-def3-11e6-bf01-fe55135034f3", "version": "24.01.000", "uri": "../lciamethods/b5c610fe-def3-11e6-bf01-fe55135034f3.xml"}, "other": {"anies": [{"value": "0.00469000713132441", "module": "A1-A3"}, {"value": "6.02358334036545E-5", "module": "C2"}, {"value": "0", "module": "C3"}, {"value": "9.21068708243148E-6", "module": "C4"}, {"value": "-0.00244913446519175", "module": "D"}, {"name": "referenceToUnitGroupDataSet", "value": {"shortDescription": [{"value": "kg NMVOC eq.", "lang": "en"}], "type": "unit group data set", "refObjectId": "d27c25f8-fbc1-44c6-b47b-4adbae4199c6", "version": "00.00.003", "uri": "../unitgroups/d27c25f8-fbc1-44c6-b47b-4adbae4199c6.xml"}}]}}, {"referenceToLCIAMethodDataSet": {"shortDescription": [{"value": "Resource use, minerals and metals", "lang": "en"}, {"value": "Potenzial für die Verknappung abiotischer Ressourcen  nicht fossile Ressourcen (ADPE)", "lang": "de"}], "type": "LCIA method data set", "refObjectId": "b2ad6494-c78d-11e6-9d9d-cec0c932ce01", "version": "24.01.000", "uri": "../lciamethods/b2ad6494-c78d-11e6-9d9d-cec0c932ce01.xml"}, "other": {"anies": [{"value": "1.16012863561264E-7", "module": "A1-A3"}, {"value": "1.71740812516029E-9", "module": "C2"}, {"value": "0", "module": "C3"}, {"value": "1.05268892733396E-10", "module": "C4"}, {"value": "-1.59153916227676E-8", "module": "D"}, {"name": "referenceToUnitGroupDataSet", "value": {"shortDescription": [{"value": "kg Sb eq.", "lang": "en"}], "type": "unit group data set", "refObjectId": "54ccd2d9-a32a-4fc2-923d-f2c8c93e89d4", "version": "25.00.000", "uri": "../unitgroups/54ccd2d9-a32a-4fc2-923d-f2c8c93e89d4.xml"}}]}}, {"referenceToLCIAMethodDataSet": {"shortDescription": [{"value": "Resource use, fossils", "lang": "en"}, {"value": "Potenzial für die Verknappung abiotischer Ressourcen  fossile Brennstoffe (ADPF)", "lang": "de"}], "type": "LCIA method data set", "refObjectId": "b2ad6110-c78d-11e6-9d9d-cec0c932ce01", "version": "24.01.000", "uri": "../lciamethods/b2ad6110-c78d-11e6-9d9d-cec0c932ce01.xml"}, "other": {"anies": [{"value": "22.7591348712647", "module": "A1-A3"}, {"value": "0.126742441960125", "module": "C2"}, {"value": "0", "module": "C3"}, {"value": "0.0217077396352839", "module": "C4"}, {"value": "-10.0892265216876", "module": "D"}, {"name": "referenceToUnitGroupDataSet", "value": {"shortDescription": [{"value": "MJ", "lang": "en"}], "type": "unit group data set", "refObjectId": "93a60a57-a3c8-11da-a746-0800200c9a66", "version": "02.00.000", "uri": "../unitgroups/93a60a57-a3c8-11da-a746-0800200c9a66.xml"}}]}}, {"referenceToLCIAMethodDataSet": {"shortDescription": [{"value": "Water use", "lang": "en"}, {"value": "Wasser-Entzugspotenzial (Benutzer) (WDP)", "lang": "de"}], "type": "LCIA method data set", "refObjectId": "b2ad66ce-c78d-11e6-9d9d-cec0c932ce01", "version": "24.01.000", "uri": "../lciamethods/b2ad66ce-c78d-11e6-9d9d-cec0c932ce01.xml"}, "other": {"anies": [{"value": "0.0313181878266405", "module": "A1-A3"}, {"value": "0.000127106529266554", "module": "C2"}, {"value": "0", "module": "C3"}, {"value": "0.000187929709708669", "module": "C4"}, {"value": "-0.0110611476188927", "module": "D"}, {"name": "referenceToUnitGroupDataSet", "value": {"shortDescription": [{"value": "m³ world equiv.", "lang": "en"}], "type": "unit group data set", "refObjectId": "6ae2df01-888e-46c8-b17d-49fa3869b476", "version": "00.00.003", "uri": "../unitgroups/6ae2df01-888e-46c8-b17d-49fa3869b476.xml"}}]}}]}, "otherAttributes": {"{http://www.indata.network/EPD/2019}epd-version": "1.2"}, "version": "1.1", "locations": "../ILCDLocations.xml"}