{"processInformation": {"dataSetInformation": {"UUID": "44d20812-1ed2-4e11-9cf0-54a3b7eb56fa", "name": {"baseName": [{"value": "FOAMGLAS® T3+", "lang": "en"}], "functionalUnitFlowProperties": [{"lang": "en"}]}, "classificationInformation": {"classification": [{"class": [{"value": "Dämmstoffe", "level": 0, "classId": "2"}, {"value": "Schaumglas", "level": 1, "classId": "2.6"}, {"value": "Platten", "level": 2, "classId": "2.6.01"}], "name": "OEKOBAU.DAT"}, {"class": [{"value": "02 Building products", "level": 0}, {"value": "Thermal insulation products", "level": 1}, {"value": "Mineral insulating materials", "level": 2}], "name": "IBUCategories"}]}, "generalComment": [{"value": "FOAMGLAS® T3+ is an insulation product for buildings made of cellular glass. It is applied to the desired dimensions in the form of slabs, panels, or other specific elements. The FOAMGLAS® T3+ is in general unfaced as a slab. In some cases, depending on the end-use, the slabs can be faced with bitumen on the top with a PE-foil (e.g. READY, BOARDS) or a white mineral liner (ROOFBLOCK, ROOF BOARDS). Also, on the bottom, the white mineral liner can be applied (cf. BOARDS).\n\nThe product is declared with a density of 95 kg/m³ (±15%) and is supplied in thicknesses of 40 mm to 200 mm.\n\nFor the placing on the market of the product FOAMGLAS® T3+ in the European Union/European Free Trade Association (EU/EFTA) (with the exception of Switzerland) Construction Products Regulation (CPR) applies. The product declaration of performance (DOP) is taking into consideration EN 13167:2015 Thermal insulation products for buildings – Factory made cellular glass (CG) products – Specification\n\nand the CE-marking. \n\n\nFor the application and use the respective national provisions apply.", "lang": "en"}], "other": {"anies": [{"scenario": [{"description": [{"value": "Landfill", "lang": "en"}], "name": "S1"}, {"description": [{"value": "Reuse", "lang": "en"}], "name": "S2"}, {"description": [{"value": "Recycle", "lang": "en"}], "name": "S3"}]}]}}, "quantitativeReference": {"referenceToReferenceFlow": [0]}, "time": {"referenceYear": 2021, "dataSetValidUntil": 2026, "other": {"anies": [{"name": "publicationDateOfEPD", "value": 1615766400000}]}}, "geography": {"locationOfOperationSupplyOrProduction": {"location": "RER"}}, "technology": {"technologyDescriptionAndIncludedProcesses": [{"value": "The product is made following the protocol of the company. All glass constituents (recycled glass, sand, sodium carbonate, feldspar, sodium sulfate, sodium nitrate, iron oxide, and FOAMGLAS®-scrap) are melted (at ca. 1250°C) in the furnace and drawn into the shape of a thin-walled tube to enable efficient grinding. Melted glass from the melter furnace is put in grinders to produce fine glass powder. In the grinding process, additives are added so that afterwards, glass foaming processes can be envisaged. In the foaming furnace, cellular glass blocks are made in moulds by heating (sintering towards ca 850°C) the glass powder after the grinding process. After the foaming process, the annealing process starts by moving the foamed blocks on the lehr where they cool according to a precisely determined curve. The cooled blocks are cut into rectangular blocks and if necessary, ground or cut to thinner sizes. The produced material is released, labelled, marked, and packed for commercialisation and various end-use applications (roof, wall, facade and other construction elements). 1 Mixing and batching of the raw materials: Recycled glass, feldspar, sodium carbonate, iron oxide, manganese oxide, sodium sulphate, sodium nitrate. 2 The melting furnace has a constant temperature of 1250°C. 3 Molten glass is drawn out of the furnace. 4 Control room for monitoring the production. 5 The glass is drawn off and falls onto the conveyor band where it cools down before entering the ball mill. 6 Addition of \"carbon black\". 7 Ball mill grinds all ingredients into a fine powder before putting them into stainless steel moulds. 8 The filled moulds pass through a cellulating oven (foaming furnace) with a temperature of 850°C. This is where the material gains its unique cell structure. 9 Energy recovery of heat. 10 The FOAMGLAS® blocks pass through an annealing oven to allow carefully controlled cooling without thermal stress. 11 The blocks are cut to size and sorted by batch. Production waste is recycled. 12 FOAMGLAS® slabs are then packaged, labelled and palletized. 13 Finished FOAMGLAS® products are stored and prepared for transport. Quality assurance Quality is assured through internal and external monitoring. The product complies with the Declaration of Performance. It also bears the CEN Keymark \nTechnical data: \nThe technical specifications of FOAMGLAS® T3+  within the scope of this EPD and within the CE marking, is according to EN 13167 and EN 14305.\n\nVoluntary data: CEN KEYMARK certificate n°001-BK-516-001; ATG H539; KOMO-CTG100-9; SIA CH672-13; ACERMI16-023-1179; Natureplus n°Zt-PCE-0406-1101-101 \nDeclared unit: \nThe Declaration refers to the life cycle of 1kg FOAMGLAS® T3 +. The gross density of the product is 95 kg / m³ ± 15%", "lang": "en"}], "technologicalApplicability": [{"value": "FOAMGLAS® T3+ products are used for roof, facades, interior, in contact with the ground, or specific insulation.", "lang": "en"}]}}, "modellingAndValidation": {"LCIMethodAndAllocation": {"typeOfDataSet": "EPD", "referenceToLCAMethodDetails": [{"shortDescription": [{"value": "Mineral insulating materials.pdf", "lang": "en"}], "type": "source data set", "refObjectId": "68e6be0e-5df5-4202-99db-e9f1e314da97"}], "other": {"anies": [{"name": "subType", "value": "specific dataset"}]}}, "dataSourcesTreatmentAndRepresentativeness": {"referenceToDataSource": [{"shortDescription": [{"value": "GaBi Database (all versions)", "lang": "en"}], "type": "source data set", "refObjectId": "28d74cc0-db8b-4d7e-bc44-5f6d56ce0c4a"}, {"shortDescription": [{"value": "GaBi database SP40 2020", "lang": "en"}], "type": "source data set", "refObjectId": "0115289e-52f0-4920-bc7e-57b1c96aec8d"}], "useAdviceForDataSet": [{"value": "Scope: \nThis document refers to the production of 1 kg uncoated \"FOAMGLAS® T3+\" cellular glass manufactured in Belgium at Tessenderlo and in Czech Republic at the Klasterec production facilities of Pittsburgh Corning Europe NV. The reference year of production is 2019. The environmental impacts of the coated product \"FOAMGLAS® T3+ in boards & blocks\" are to be assessed with the help of a markup factor in the amount of 0.8% for Global Warming Potential. \nSystem boundary: \nType of EPD: Cradle to Grave with options, modules C1-C4, and module D (A1-A3, C, D and additional modules) \n\nThe LCA addresses the life cycle stage of production, installation, end-of-life (EoL) and potential benefits beyond the system boundaries. \n\nThe product stage comprises of modules A1 (raw material supply), A2 (transport) and A3 (production). The following individual processes were included in the product stage A1- A3 of production:\n\nProcesses for providing preliminary products and energy\nTransporting the raw materials and preliminary materials to the plant\nThe manufacturing process in the plant including energy-related expenses, disposal of residual materials and emissions\nProduction of packaging\n\n\nModule A4 takes into account the transportation of product to the construction site. The treatment of the packaging materials is assigned to module A5 . Module C1 takes into accounts the de-construction or demolition of the product before taking it for treatment/disposal through means of transportation (module C2). Module C3 is the waste processing of the product before recycling/recovery/reuse. Landfilling with residual materials is assigned to module C4 . Module D accounts for the potential credits resulting from the thermal and electrical energy generated when burning packaging materials in module A5 (energy substitution).\n\nThere are 3 EoL scenarios in the study: Landfill, Reuse and Recycling. Module D/2 takes into account potential credits for 100% reuse of material and module D/3 considers potential credits for replacing kaolin in the brick industry.", "lang": "en"}], "other": {"anies": [{"name": "referenceToOriginalEPD", "value": {"shortDescription": {"value": "FOAMGLAS® T3+.pdf", "defaultValue": "FOAMGLAS® T3+.pdf", "lstrings": [{"lang": "en", "value": "FOAMGLAS® T3+.pdf"}]}, "type": "source data set", "uuid": {"uuid": "ef4cc465-aaef-44d5-9a7c-74a82239d00e"}, "refObjectId": "ef4cc465-aaef-44d5-9a7c-74a82239d00e", "resourceURLs": ["https://oekobaudat.de/OEKOBAU.DAT/resource/sources/ef4cc465-aaef-44d5-9a7c-74a82239d00e/FOAMGLAS_T3__15561.pdf?version=00.01.000"]}}]}}, "validation": {"review": [{"referenceToNameOfReviewerAndInstitution": [{"shortDescription": [{"value": "Institut Bauen und Umwelt e. V.", "lang": "en"}], "type": "contact data set", "refObjectId": "d111dbec-b024-4be5-86c5-752d6eb2cf95", "uri": "../contacts/d111dbec-b024-4be5-86c5-752d6eb2cf95.xml"}], "type": "Accredited third party review"}]}, "complianceDeclarations": {"compliance": [{"referenceToComplianceSystem": {"shortDescription": [{"value": "DIN EN 15804+A2", "lang": "en"}], "type": "source data set", "refObjectId": "c0016b33-8cf7-415c-ac6e-deba0d21440d", "uri": "../sources/c0016b33-8cf7-415c-ac6e-deba0d21440d.xml"}}, {"referenceToComplianceSystem": {"shortDescription": [{"value": "ISO 14025", "lang": "en"}], "type": "source data set", "refObjectId": "4f2eb655-6e44-4874-a95a-e28f5442cd4d", "uri": "../sources/4f2eb655-6e44-4874-a95a-e28f5442cd4d.xml"}}]}}, "administrativeInformation": {"commissionerAndGoal": {"referenceToCommissioner": [{"shortDescription": [{"value": "Pittsburgh Corning Europe NV", "lang": "en"}], "type": "contact data set", "refObjectId": "7decf5ec-2592-44cc-b676-fa81bb05cf72", "uri": "../contacts/7decf5ec-2592-44cc-b676-fa81bb05cf72.xml"}]}, "dataGenerator": {"referenceToPersonOrEntityGeneratingTheDataSet": [{"shortDescription": [{"value": "Sphera Solutions GmbH", "lang": "en"}], "type": "contact data set", "refObjectId": "623edf96-39d1-4e6f-9892-674c7228546b", "uri": "../contacts/623edf96-39d1-4e6f-9892-674c7228546b.xml"}]}, "dataEntryBy": {"timeStamp": 1615766400000, "referenceToDataSetFormat": [{"shortDescription": [{"value": "ILCD Format", "lang": "en"}], "type": "source data set", "refObjectId": "a97a0155-0234-4b87-b4ce-a45da52f2a40", "uri": "../sources/a97a0155-0234-4b87-b4ce-a45da52f2a40.xml"}, {"shortDescription": [{"value": "EPD-Datenformaterweiterungen v1.2", "lang": "de"}, {"value": "EPD Data Format Extensions v1.2", "lang": "en"}], "type": "source data set", "refObjectId": "a29449fd-aa2f-4de8-b5d7-4b06b43c6fde", "uri": "../sources/a29449fd-aa2f-4de8-b5d7-4b06b43c6fde.xml"}]}, "publicationAndOwnership": {"dataSetVersion": "00.01.000", "referenceToPrecedingDataSetVersion": [{"shortDescription": [{"value": "FOAMGLAS® T3+", "lang": "en"}], "type": "process data set", "refObjectId": "f8ff7cbf-f3bb-4499-95e2-8268dd84fab1", "uri": "../processes/f8ff7cbf-f3bb-4499-95e2-8268dd84fab1.xml"}], "referenceToRegistrationAuthority": {"shortDescription": [{"value": "Institut Bauen und Umwelt e. V.", "lang": "en"}], "type": "contact data set", "refObjectId": "d111dbec-b024-4be5-86c5-752d6eb2cf95", "uri": "../contacts/d111dbec-b024-4be5-86c5-752d6eb2cf95.xml"}, "registrationNumber": "EPD-PCE-20200300-IBB2-EN", "referenceToOwnershipOfDataSet": {"shortDescription": [{"value": "Pittsburgh Corning Europe NV", "lang": "en"}], "type": "contact data set", "refObjectId": "7decf5ec-2592-44cc-b676-fa81bb05cf72", "uri": "../contacts/7decf5ec-2592-44cc-b676-fa81bb05cf72.xml"}, "copyright": true, "licenseType": "Free of charge for all users and uses", "accessRestrictions": [{"value": "None", "lang": "en"}], "other": {"anies": [{"name": "referenceToPublisher", "value": {"shortDescription": [{"value": "Institut Bauen und Umwelt e. V.", "lang": "en"}], "type": "contact data set", "refObjectId": "d111dbec-b024-4be5-86c5-752d6eb2cf95", "uri": "../contacts/d111dbec-b024-4be5-86c5-752d6eb2cf95.xml"}}]}}}, "exchanges": {"exchange": [{"dataSetInternalID": 0, "referenceToFlowDataSet": {"shortDescription": [{"value": "FOAMGLAS® T3+ (1 kg FOAMGLAS® W+F bzw. FOAMGLAS® T3+)", "lang": "en"}], "type": "flow data set", "refObjectId": "eb3c424c-97f4-ff0b-ab3e-71a64d2c9d66", "uri": "../flows/eb3c424c-97f4-ff0b-ab3e-71a64d2c9d66.xml"}, "meanAmount": 1.0, "referencesToDataSource": {}, "referenceFlow": true, "resolvedFlowVersion": "00.05.000", "resultingflowAmount": 1.0, "flowProperties": [{"name": [{"lang": "en", "value": "Mass"}, {"lang": "de", "value": "Masse"}], "uuid": "93a60a56-a3c8-11da-a746-0800200b9a66", "referenceFlowProperty": true, "meanValue": 1.0, "referenceUnit": "kg", "unitGroupUUID": "ad38d542-3fe9-439d-9b95-2f5f7752acaf"}], "materialProperties": [{"name": "gross density", "value": "100.0", "unit": "kg/m^3", "unitDescription": "kilograms per cubic metre"}], "typeOfFlow": "Product flow", "classification": {"classHierarchy": "Dämmstoffe / Schaumglas / Platten", "name": "OEKOBAU.DAT"}}, {"dataSetInternalID": 1, "referenceToFlowDataSet": {"shortDescription": [{"value": "Renewable primary energy as energy carrier (PERE)", "lang": "en"}], "type": "flow data set", "refObjectId": "20f32be5-0398-4288-9b6d-accddd195317", "uri": "../flows/20f32be5-0398-4288-9b6d-accddd195317.xml"}, "exchange direction": "INPUT", "other": {"anies": [{"name": "referenceToUnitGroupDataSet", "value": {"shortDescription": [{"value": "MJ", "lang": "en"}], "type": "unit group data set", "refObjectId": "93a60a57-a3c8-11da-a746-0800200c9a66", "uri": "../unitgroups/93a60a57-a3c8-11da-a746-0800200c9a66.xml"}}, {"value": "13.3", "module": "A1-A3"}, {"value": "0.021", "module": "A4"}, {"value": "0.61", "module": "A5"}, {"value": "0.000461", "module": "C1"}, {"value": "0.00167", "module": "C2"}, {"value": "0", "module": "C3", "scenario": "S2"}, {"value": "0.015", "module": "C3", "scenario": "S3"}, {"value": "0.0261", "module": "C4"}, {"value": "-0.177", "module": "D", "scenario": "S0"}, {"value": "-13.3", "module": "D", "scenario": "S2"}, {"value": "-0.0955", "module": "D", "scenario": "S3"}]}, "resolvedFlowVersion": "38.00.000", "flowProperties": [], "typeOfFlow": "Other flow", "classification": {"classHierarchy": "Quantities", "name": "GaBiCategories"}}, {"dataSetInternalID": 2, "referenceToFlowDataSet": {"shortDescription": [{"value": "Renewable primary energy resources as material utilization (PERM)", "lang": "en"}], "type": "flow data set", "refObjectId": "fb3ec0de-548d-4508-aea5-00b73bf6f702", "uri": "../flows/fb3ec0de-548d-4508-aea5-00b73bf6f702.xml"}, "exchange direction": "INPUT", "other": {"anies": [{"name": "referenceToUnitGroupDataSet", "value": {"shortDescription": [{"value": "MJ", "lang": "en"}], "type": "unit group data set", "refObjectId": "93a60a57-a3c8-11da-a746-0800200c9a66", "uri": "../unitgroups/93a60a57-a3c8-11da-a746-0800200c9a66.xml"}}, {"value": "0.6", "module": "A1-A3"}, {"value": "0", "module": "A4"}, {"value": "-0.6", "module": "A5"}, {"value": "0", "module": "C1"}, {"value": "0", "module": "C2"}, {"value": "0", "module": "C3", "scenario": "S2"}, {"value": "0", "module": "C3", "scenario": "S3"}, {"value": "0", "module": "C4"}, {"value": "0", "module": "D", "scenario": "S0"}, {"value": "-0.6", "module": "D", "scenario": "S2"}, {"value": "0", "module": "D", "scenario": "S3"}]}, "resolvedFlowVersion": "38.00.000", "flowProperties": [], "typeOfFlow": "Other flow", "classification": {"classHierarchy": "Quantities", "name": "GaBiCategories"}}, {"dataSetInternalID": 3, "referenceToFlowDataSet": {"shortDescription": [{"value": "Total use of renewable primary energy resources (PERT)", "lang": "en"}], "type": "flow data set", "refObjectId": "53f97275-fa8a-4cdd-9024-65936002acd0", "uri": "../flows/53f97275-fa8a-4cdd-9024-65936002acd0.xml"}, "exchange direction": "INPUT", "other": {"anies": [{"name": "referenceToUnitGroupDataSet", "value": {"shortDescription": [{"value": "MJ", "lang": "en"}], "type": "unit group data set", "refObjectId": "93a60a57-a3c8-11da-a746-0800200c9a66", "uri": "../unitgroups/93a60a57-a3c8-11da-a746-0800200c9a66.xml"}}, {"value": "13.9", "module": "A1-A3"}, {"value": "0.021", "module": "A4"}, {"value": "0.01", "module": "A5"}, {"value": "0.000461", "module": "C1"}, {"value": "0.00167", "module": "C2"}, {"value": "0", "module": "C3", "scenario": "S2"}, {"value": "0.015", "module": "C3", "scenario": "S3"}, {"value": "0.0261", "module": "C4"}, {"value": "-0.177", "module": "D", "scenario": "S0"}, {"value": "-13.9", "module": "D", "scenario": "S2"}, {"value": "-0.0955", "module": "D", "scenario": "S3"}]}, "resolvedFlowVersion": "38.00.000", "flowProperties": [], "typeOfFlow": "Other flow", "classification": {"classHierarchy": "Quantities / Environmental quantities / EPD EN 15804 / LCI indicators", "name": "GaBiCategories"}}, {"dataSetInternalID": 4, "referenceToFlowDataSet": {"shortDescription": [{"value": "Non renewable primary energy as energy carrier (PENRE)", "lang": "en"}], "type": "flow data set", "refObjectId": "ac857178-2b45-46ec-892a-a9a4332f0372", "uri": "../flows/ac857178-2b45-46ec-892a-a9a4332f0372.xml"}, "exchange direction": "INPUT", "other": {"anies": [{"name": "referenceToUnitGroupDataSet", "value": {"shortDescription": [{"value": "MJ", "lang": "en"}], "type": "unit group data set", "refObjectId": "93a60a57-a3c8-11da-a746-0800200c9a66", "uri": "../unitgroups/93a60a57-a3c8-11da-a746-0800200c9a66.xml"}}, {"value": "22.1", "module": "A1-A3"}, {"value": "0.375", "module": "A4"}, {"value": "0.932", "module": "A5"}, {"value": "0.00821", "module": "C1"}, {"value": "0.0298", "module": "C2"}, {"value": "0", "module": "C3", "scenario": "S2"}, {"value": "0.034", "module": "C3", "scenario": "S3"}, {"value": "0.199", "module": "C4"}, {"value": "-0.866", "module": "D", "scenario": "S0"}, {"value": "-22.1", "module": "D", "scenario": "S2"}, {"value": "-2.35", "module": "D", "scenario": "S3"}]}, "resolvedFlowVersion": "38.00.000", "flowProperties": [], "typeOfFlow": "Other flow", "classification": {"classHierarchy": "Quantities", "name": "GaBiCategories"}}, {"dataSetInternalID": 5, "referenceToFlowDataSet": {"shortDescription": [{"value": "Non renewable primary energy as material utilization (PENRM)", "lang": "en"}], "type": "flow data set", "refObjectId": "1421caa0-679d-4bf4-b282-0eb850ccae27", "uri": "../flows/1421caa0-679d-4bf4-b282-0eb850ccae27.xml"}, "exchange direction": "INPUT", "other": {"anies": [{"name": "referenceToUnitGroupDataSet", "value": {"shortDescription": [{"value": "MJ", "lang": "en"}], "type": "unit group data set", "refObjectId": "93a60a57-a3c8-11da-a746-0800200c9a66", "uri": "../unitgroups/93a60a57-a3c8-11da-a746-0800200c9a66.xml"}}, {"value": "0.89", "module": "A1-A3"}, {"value": "0", "module": "A4"}, {"value": "-0.89", "module": "A5"}, {"value": "0", "module": "C1"}, {"value": "0", "module": "C2"}, {"value": "0", "module": "C3", "scenario": "S2"}, {"value": "0", "module": "C3", "scenario": "S3"}, {"value": "0", "module": "C4"}, {"value": "0", "module": "D", "scenario": "S0"}, {"value": "-0.89", "module": "D", "scenario": "S2"}, {"value": "0", "module": "D", "scenario": "S3"}]}, "resolvedFlowVersion": "38.00.000", "flowProperties": [], "typeOfFlow": "Other flow", "classification": {"classHierarchy": "Quantities", "name": "GaBiCategories"}}, {"dataSetInternalID": 6, "referenceToFlowDataSet": {"shortDescription": [{"value": "Total use of non renewable primary energy resources (PENRT)", "lang": "en"}], "type": "flow data set", "refObjectId": "06159210-646b-4c8d-8583-da9b3b95a6c1", "uri": "../flows/06159210-646b-4c8d-8583-da9b3b95a6c1.xml"}, "exchange direction": "INPUT", "other": {"anies": [{"name": "referenceToUnitGroupDataSet", "value": {"shortDescription": [{"value": "MJ", "lang": "en"}], "type": "unit group data set", "refObjectId": "93a60a57-a3c8-11da-a746-0800200c9a66", "uri": "../unitgroups/93a60a57-a3c8-11da-a746-0800200c9a66.xml"}}, {"value": "22.99", "module": "A1-A3"}, {"value": "0.375", "module": "A4"}, {"value": "0.042", "module": "A5"}, {"value": "0.00821", "module": "C1"}, {"value": "0.0298", "module": "C2"}, {"value": "0", "module": "C3", "scenario": "S2"}, {"value": "0.034", "module": "C3", "scenario": "S3"}, {"value": "0.199", "module": "C4"}, {"value": "-0.866", "module": "D", "scenario": "S0"}, {"value": "-22.99", "module": "D", "scenario": "S2"}, {"value": "-2.35", "module": "D", "scenario": "S3"}]}, "resolvedFlowVersion": "38.00.000", "flowProperties": [], "typeOfFlow": "Other flow", "classification": {"classHierarchy": "Quantities / Environmental quantities / EPD EN 15804 / LCI indicators", "name": "GaBiCategories"}}, {"dataSetInternalID": 7, "referenceToFlowDataSet": {"shortDescription": [{"value": "Use of secondary material (SM)", "lang": "en"}], "type": "flow data set", "refObjectId": "c6a1f35f-2d09-4f54-8dfb-97e502e1ce92", "uri": "../flows/c6a1f35f-2d09-4f54-8dfb-97e502e1ce92.xml"}, "exchange direction": "INPUT", "other": {"anies": [{"name": "referenceToUnitGroupDataSet", "value": {"shortDescription": [{"value": "kg", "lang": "en"}], "type": "unit group data set", "refObjectId": "ad38d542-3fe9-439d-9b95-2f5f7752acaf", "uri": "../unitgroups/ad38d542-3fe9-439d-9b95-2f5f7752acaf.xml"}}, {"value": "0.56", "module": "A1-A3"}, {"value": "0", "module": "A4"}, {"value": "0", "module": "A5"}, {"value": "0", "module": "C1"}, {"value": "0", "module": "C2"}, {"value": "0", "module": "C3", "scenario": "S2"}, {"value": "0", "module": "C3", "scenario": "S3"}, {"value": "0", "module": "C4"}, {"value": "0", "module": "D", "scenario": "S0"}, {"value": "0", "module": "D", "scenario": "S2"}, {"value": "0", "module": "D", "scenario": "S3"}]}, "resolvedFlowVersion": "38.00.000", "flowProperties": [], "typeOfFlow": "Other flow", "classification": {"classHierarchy": "Quantities / Environmental quantities / EPD EN 15804 / LCI indicators", "name": "GaBiCategories"}}, {"dataSetInternalID": 8, "referenceToFlowDataSet": {"shortDescription": [{"value": "Use of renewable secondary fuels (RSF)", "lang": "en"}], "type": "flow data set", "refObjectId": "64333088-a55f-4aa2-9a31-c10b07816787", "uri": "../flows/64333088-a55f-4aa2-9a31-c10b07816787.xml"}, "exchange direction": "INPUT", "other": {"anies": [{"name": "referenceToUnitGroupDataSet", "value": {"shortDescription": [{"value": "MJ", "lang": "en"}], "type": "unit group data set", "refObjectId": "93a60a57-a3c8-11da-a746-0800200c9a66", "uri": "../unitgroups/93a60a57-a3c8-11da-a746-0800200c9a66.xml"}}, {"value": "0", "module": "A1-A3"}, {"value": "0", "module": "A4"}, {"value": "0", "module": "A5"}, {"value": "0", "module": "C1"}, {"value": "0", "module": "C2"}, {"value": "0", "module": "C3", "scenario": "S2"}, {"value": "0", "module": "C3", "scenario": "S3"}, {"value": "0", "module": "C4"}, {"value": "0", "module": "D", "scenario": "S0"}, {"value": "0", "module": "D", "scenario": "S2"}, {"value": "0", "module": "D", "scenario": "S3"}]}, "resolvedFlowVersion": "38.00.000", "flowProperties": [], "typeOfFlow": "Other flow", "classification": {"classHierarchy": "Quantities / Environmental quantities / EPD EN 15804 / LCI indicators", "name": "GaBiCategories"}}, {"dataSetInternalID": 9, "referenceToFlowDataSet": {"shortDescription": [{"value": "Use of non renewable secondary fuels (NRSF)", "lang": "en"}], "type": "flow data set", "refObjectId": "89def144-d39a-4287-b86f-efde453ddcb2", "uri": "../flows/89def144-d39a-4287-b86f-efde453ddcb2.xml"}, "exchange direction": "INPUT", "other": {"anies": [{"name": "referenceToUnitGroupDataSet", "value": {"shortDescription": [{"value": "MJ", "lang": "en"}], "type": "unit group data set", "refObjectId": "93a60a57-a3c8-11da-a746-0800200c9a66", "uri": "../unitgroups/93a60a57-a3c8-11da-a746-0800200c9a66.xml"}}, {"value": "0", "module": "A1-A3"}, {"value": "0", "module": "A4"}, {"value": "0", "module": "A5"}, {"value": "0", "module": "C1"}, {"value": "0", "module": "C2"}, {"value": "0", "module": "C3", "scenario": "S2"}, {"value": "0", "module": "C3", "scenario": "S3"}, {"value": "0", "module": "C4"}, {"value": "0", "module": "D", "scenario": "S0"}, {"value": "0", "module": "D", "scenario": "S2"}, {"value": "0", "module": "D", "scenario": "S3"}]}, "resolvedFlowVersion": "38.00.000", "flowProperties": [], "typeOfFlow": "Other flow", "classification": {"classHierarchy": "Quantities / Environmental quantities / EPD EN 15804 / LCI indicators", "name": "GaBiCategories"}}, {"dataSetInternalID": 10, "referenceToFlowDataSet": {"shortDescription": [{"value": "Use of net fresh water (FW)", "lang": "en"}], "type": "flow data set", "refObjectId": "3cf952c8-f3a4-461d-8c96-96456ca62246", "uri": "../flows/3cf952c8-f3a4-461d-8c96-96456ca62246.xml"}, "exchange direction": "INPUT", "other": {"anies": [{"name": "referenceToUnitGroupDataSet", "value": {"shortDescription": [{"value": "m^3", "lang": "en"}], "type": "unit group data set", "refObjectId": "cd950537-0a98-4044-9ba7-9f9a68d0a504", "uri": "../unitgroups/cd950537-0a98-4044-9ba7-9f9a68d0a504.xml"}}, {"value": "0.0394", "module": "A1-A3"}, {"value": "2.44E-05", "module": "A4"}, {"value": "0.000306", "module": "A5"}, {"value": "5.34E-07", "module": "C1"}, {"value": "1.94E-06", "module": "C2"}, {"value": "0", "module": "C3", "scenario": "S2"}, {"value": "1.74E-05", "module": "C3", "scenario": "S3"}, {"value": "5.02E-05", "module": "C4"}, {"value": "-0.000205", "module": "D", "scenario": "S0"}, {"value": "-0.0394", "module": "D", "scenario": "S2"}, {"value": "-0.000112", "module": "D", "scenario": "S3"}]}, "resolvedFlowVersion": "38.00.000", "flowProperties": [], "typeOfFlow": "Other flow", "classification": {"classHierarchy": "Quantities / Environmental quantities / EPD EN 15804 / LCI indicators", "name": "GaBiCategories"}}, {"dataSetInternalID": 11, "referenceToFlowDataSet": {"shortDescription": [{"value": "Hazardous waste disposed (HWD)", "lang": "en"}], "type": "flow data set", "refObjectId": "430f9e0f-59b2-46a0-8e0d-55e0e84948fc", "uri": "../flows/430f9e0f-59b2-46a0-8e0d-55e0e84948fc.xml"}, "exchange direction": "OUTPUT", "other": {"anies": [{"name": "referenceToUnitGroupDataSet", "value": {"shortDescription": [{"value": "kg", "lang": "en"}], "type": "unit group data set", "refObjectId": "ad38d542-3fe9-439d-9b95-2f5f7752acaf", "uri": "../unitgroups/ad38d542-3fe9-439d-9b95-2f5f7752acaf.xml"}}, {"value": "4.96E-08", "module": "A1-A3"}, {"value": "1.74E-08", "module": "A4"}, {"value": "1.14E-10", "module": "A5"}, {"value": "3.82E-10", "module": "C1"}, {"value": "1.39E-09", "module": "C2"}, {"value": "0", "module": "C3", "scenario": "S2"}, {"value": "1.41E-11", "module": "C3", "scenario": "S3"}, {"value": "3.03E-09", "module": "C4"}, {"value": "-3.44E-10", "module": "D", "scenario": "S0"}, {"value": "-4.96E-08", "module": "D", "scenario": "S2"}, {"value": "-1.98E-09", "module": "D", "scenario": "S3"}]}, "resolvedFlowVersion": "38.00.000", "flowProperties": [], "typeOfFlow": "Other flow", "classification": {"classHierarchy": "Quantities / Environmental quantities / EPD EN 15804 / LCI indicators", "name": "GaBiCategories"}}, {"dataSetInternalID": 12, "referenceToFlowDataSet": {"shortDescription": [{"value": "Non hazardous waste disposed (NHWD)", "lang": "en"}], "type": "flow data set", "refObjectId": "b29ef66b-e286-4afa-949f-62f1a7b4d7fa", "uri": "../flows/b29ef66b-e286-4afa-949f-62f1a7b4d7fa.xml"}, "exchange direction": "OUTPUT", "other": {"anies": [{"name": "referenceToUnitGroupDataSet", "value": {"shortDescription": [{"value": "kg", "lang": "en"}], "type": "unit group data set", "refObjectId": "ad38d542-3fe9-439d-9b95-2f5f7752acaf", "uri": "../unitgroups/ad38d542-3fe9-439d-9b95-2f5f7752acaf.xml"}}, {"value": "0.0412", "module": "A1-A3"}, {"value": "5.74E-05", "module": "A4"}, {"value": "0.00669", "module": "A5"}, {"value": "1.26E-06", "module": "C1"}, {"value": "4.56E-06", "module": "C2"}, {"value": "0", "module": "C3", "scenario": "S2"}, {"value": "2.41E-05", "module": "C3", "scenario": "S3"}, {"value": "1", "module": "C4"}, {"value": "-0.000386", "module": "D", "scenario": "S0"}, {"value": "-0.0412", "module": "D", "scenario": "S2"}, {"value": "-0.000623", "module": "D", "scenario": "S3"}]}, "resolvedFlowVersion": "38.00.000", "flowProperties": [], "typeOfFlow": "Other flow", "classification": {"classHierarchy": "Quantities / Environmental quantities / EPD EN 15804 / LCI indicators", "name": "GaBiCategories"}}, {"dataSetInternalID": 13, "referenceToFlowDataSet": {"shortDescription": [{"value": "Radioactive waste disposed (RWD)", "lang": "en"}], "type": "flow data set", "refObjectId": "3449546e-52ad-4b39-b809-9fb77cea8ff6", "uri": "../flows/3449546e-52ad-4b39-b809-9fb77cea8ff6.xml"}, "exchange direction": "OUTPUT", "other": {"anies": [{"name": "referenceToUnitGroupDataSet", "value": {"shortDescription": [{"value": "kg", "lang": "en"}], "type": "unit group data set", "refObjectId": "ad38d542-3fe9-439d-9b95-2f5f7752acaf", "uri": "../unitgroups/ad38d542-3fe9-439d-9b95-2f5f7752acaf.xml"}}, {"value": "0.000109", "module": "A1-A3"}, {"value": "4.64E-07", "module": "A4"}, {"value": "1.85E-06", "module": "A5"}, {"value": "1.02E-08", "module": "C1"}, {"value": "3.68E-08", "module": "C2"}, {"value": "0", "module": "C3", "scenario": "S2"}, {"value": "5.15E-06", "module": "C3", "scenario": "S3"}, {"value": "2.26E-06", "module": "C4"}, {"value": "-6.03E-05", "module": "D", "scenario": "S0"}, {"value": "-0.000109", "module": "D", "scenario": "S2"}, {"value": "-3.14E-05", "module": "D", "scenario": "S3"}]}, "resolvedFlowVersion": "38.00.000", "flowProperties": [], "typeOfFlow": "Other flow", "classification": {"classHierarchy": "Quantities / Environmental quantities / EPD EN 15804 / LCI indicators", "name": "GaBiCategories"}}, {"dataSetInternalID": 14, "referenceToFlowDataSet": {"shortDescription": [{"value": "Components for re-use (CRU)", "lang": "en"}], "type": "flow data set", "refObjectId": "a2b32f97-3fc7-4af2-b209-525bc6426f33", "uri": "../flows/a2b32f97-3fc7-4af2-b209-525bc6426f33.xml"}, "exchange direction": "OUTPUT", "other": {"anies": [{"name": "referenceToUnitGroupDataSet", "value": {"shortDescription": [{"value": "kg", "lang": "en"}], "type": "unit group data set", "refObjectId": "ad38d542-3fe9-439d-9b95-2f5f7752acaf", "uri": "../unitgroups/ad38d542-3fe9-439d-9b95-2f5f7752acaf.xml"}}, {"value": "0", "module": "A1-A3"}, {"value": "0", "module": "A4"}, {"value": "0", "module": "A5"}, {"value": "0", "module": "C1"}, {"value": "0", "module": "C2"}, {"value": "1", "module": "C3", "scenario": "S2"}, {"value": "0", "module": "C3", "scenario": "S3"}, {"value": "0", "module": "C4"}, {"value": "0", "module": "D", "scenario": "S0"}, {"value": "0", "module": "D", "scenario": "S2"}, {"value": "0", "module": "D", "scenario": "S3"}]}, "resolvedFlowVersion": "38.00.000", "flowProperties": [], "typeOfFlow": "Other flow", "classification": {"classHierarchy": "Quantities / Environmental quantities / EPD EN 15804 / LCI indicators", "name": "GaBiCategories"}}, {"dataSetInternalID": 15, "referenceToFlowDataSet": {"shortDescription": [{"value": "Materials for recycling (MFR)", "lang": "en"}], "type": "flow data set", "refObjectId": "d7fe48a5-4103-49c8-9aae-b0b5dfdbd6ae", "uri": "../flows/d7fe48a5-4103-49c8-9aae-b0b5dfdbd6ae.xml"}, "exchange direction": "OUTPUT", "other": {"anies": [{"name": "referenceToUnitGroupDataSet", "value": {"shortDescription": [{"value": "kg", "lang": "en"}], "type": "unit group data set", "refObjectId": "ad38d542-3fe9-439d-9b95-2f5f7752acaf", "uri": "../unitgroups/ad38d542-3fe9-439d-9b95-2f5f7752acaf.xml"}}, {"value": "0", "module": "A1-A3"}, {"value": "0", "module": "A4"}, {"value": "0", "module": "A5"}, {"value": "0", "module": "C1"}, {"value": "0", "module": "C2"}, {"value": "0", "module": "C3", "scenario": "S2"}, {"value": "0.44", "module": "C3", "scenario": "S3"}, {"value": "0", "module": "C4"}, {"value": "0", "module": "D", "scenario": "S0"}, {"value": "0", "module": "D", "scenario": "S2"}, {"value": "0", "module": "D", "scenario": "S3"}]}, "resolvedFlowVersion": "38.00.000", "flowProperties": [], "typeOfFlow": "Other flow", "classification": {"classHierarchy": "Quantities / Environmental quantities / EPD EN 15804 / LCI indicators", "name": "GaBiCategories"}}, {"dataSetInternalID": 16, "referenceToFlowDataSet": {"shortDescription": [{"value": "Materials for energy recovery (MER)", "lang": "en"}], "type": "flow data set", "refObjectId": "59a9181c-3aaf-46ee-8b13-2b3723b6e447", "uri": "../flows/59a9181c-3aaf-46ee-8b13-2b3723b6e447.xml"}, "exchange direction": "OUTPUT", "other": {"anies": [{"name": "referenceToUnitGroupDataSet", "value": {"shortDescription": [{"value": "kg", "lang": "en"}], "type": "unit group data set", "refObjectId": "ad38d542-3fe9-439d-9b95-2f5f7752acaf", "uri": "../unitgroups/ad38d542-3fe9-439d-9b95-2f5f7752acaf.xml"}}, {"value": "0", "module": "A1-A3"}, {"value": "0", "module": "A4"}, {"value": "0.0609", "module": "A5"}, {"value": "0", "module": "C1"}, {"value": "0", "module": "C2"}, {"value": "0", "module": "C3", "scenario": "S2"}, {"value": "0", "module": "C3", "scenario": "S3"}, {"value": "0", "module": "C4"}, {"value": "0", "module": "D", "scenario": "S0"}, {"value": "0", "module": "D", "scenario": "S2"}, {"value": "0", "module": "D", "scenario": "S3"}]}, "resolvedFlowVersion": "38.00.000", "flowProperties": [], "typeOfFlow": "Other flow", "classification": {"classHierarchy": "Quantities / Environmental quantities / EPD EN 15804 / LCI indicators", "name": "GaBiCategories"}}, {"dataSetInternalID": 17, "referenceToFlowDataSet": {"shortDescription": [{"value": "Exported electrical energy (EEE)", "lang": "en"}], "type": "flow data set", "refObjectId": "4da0c987-2b76-40d6-9e9e-82a017aaaf29", "uri": "../flows/4da0c987-2b76-40d6-9e9e-82a017aaaf29.xml"}, "exchange direction": "OUTPUT", "other": {"anies": [{"name": "referenceToUnitGroupDataSet", "value": {"shortDescription": [{"value": "MJ", "lang": "en"}], "type": "unit group data set", "refObjectId": "93a60a57-a3c8-11da-a746-0800200c9a66", "uri": "../unitgroups/93a60a57-a3c8-11da-a746-0800200c9a66.xml"}}, {"value": "0", "module": "A1-A3"}, {"value": "0", "module": "A4"}, {"value": "0.202", "module": "A5"}, {"value": "0", "module": "C1"}, {"value": "0", "module": "C2"}, {"value": "0", "module": "C3", "scenario": "S2"}, {"value": "0", "module": "C3", "scenario": "S3"}, {"value": "0", "module": "C4"}, {"value": "0", "module": "D", "scenario": "S0"}, {"value": "0", "module": "D", "scenario": "S2"}, {"value": "0", "module": "D", "scenario": "S3"}]}, "resolvedFlowVersion": "38.00.000", "flowProperties": [], "typeOfFlow": "Other flow", "classification": {"classHierarchy": "Quantities / Environmental quantities / EPD EN 15804 / LCI indicators", "name": "GaBiCategories"}}, {"dataSetInternalID": 18, "referenceToFlowDataSet": {"shortDescription": [{"value": "Exported thermal energy (EET)", "lang": "en"}], "type": "flow data set", "refObjectId": "98daf38a-7a79-46d3-9a37-2b7bd0955810", "uri": "../flows/98daf38a-7a79-46d3-9a37-2b7bd0955810.xml"}, "exchange direction": "OUTPUT", "other": {"anies": [{"name": "referenceToUnitGroupDataSet", "value": {"shortDescription": [{"value": "MJ", "lang": "en"}], "type": "unit group data set", "refObjectId": "93a60a57-a3c8-11da-a746-0800200c9a66", "uri": "../unitgroups/93a60a57-a3c8-11da-a746-0800200c9a66.xml"}}, {"value": "0", "module": "A1-A3"}, {"value": "0", "module": "A4"}, {"value": "0.415", "module": "A5"}, {"value": "0", "module": "C1"}, {"value": "0", "module": "C2"}, {"value": "0", "module": "C3", "scenario": "S2"}, {"value": "0", "module": "C3", "scenario": "S3"}, {"value": "0", "module": "C4"}, {"value": "0", "module": "D", "scenario": "S0"}, {"value": "0", "module": "D", "scenario": "S2"}, {"value": "0", "module": "D", "scenario": "S3"}]}, "resolvedFlowVersion": "38.00.000", "flowProperties": [], "typeOfFlow": "Other flow", "classification": {"classHierarchy": "Quantities / Environmental quantities / EPD EN 15804 / LCI indicators", "name": "GaBiCategories"}}]}, "LCIAResults": {"LCIAResult": [{"referenceToLCIAMethodDataSet": {"shortDescription": [{"value": "Global Warming Potential total (GWP-total)", "lang": "en"}], "type": "LCIA method data set", "refObjectId": "6a37f984-a4b3-458a-a20a-64418c145fa2", "uri": "../lciamethods/6a37f984-a4b3-458a-a20a-64418c145fa2.xml"}, "other": {"anies": [{"name": "referenceToUnitGroupDataSet", "value": {"shortDescription": [{"value": "kg CO_(2)-Äq.", "lang": "en"}], "type": "unit group data set", "refObjectId": "1ebf3012-d0db-4de2-aefd-ef30cedb0be1", "uri": "../unitgroups/1ebf3012-d0db-4de2-aefd-ef30cedb0be1.xml"}}, {"value": "1.4536", "module": "A1-A3"}, {"value": "0.0296", "module": "A4"}, {"value": "0.123", "module": "A5"}, {"value": "0.000647", "module": "C1"}, {"value": "0.00235", "module": "C2"}, {"value": "0", "module": "C3", "scenario": "S2"}, {"value": "0.00195", "module": "C3", "scenario": "S3"}, {"value": "0.01529", "module": "C4"}, {"value": "-0.0513", "module": "D", "scenario": "S0"}, {"value": "-1.4536", "module": "D", "scenario": "S2"}, {"value": "-0.143", "module": "D", "scenario": "S3"}]}}, {"referenceToLCIAMethodDataSet": {"shortDescription": [{"value": "Global Warming Potential fossil fuels (GWP-fossil)", "lang": "en"}], "type": "LCIA method data set", "refObjectId": "5f635281-343e-44fb-83df-1971b155e6b6", "uri": "../lciamethods/5f635281-343e-44fb-83df-1971b155e6b6.xml"}, "other": {"anies": [{"name": "referenceToUnitGroupDataSet", "value": {"shortDescription": [{"value": "kg CO_(2)-Äq.", "lang": "en"}], "type": "unit group data set", "refObjectId": "1ebf3012-d0db-4de2-aefd-ef30cedb0be1", "uri": "../unitgroups/1ebf3012-d0db-4de2-aefd-ef30cedb0be1.xml"}}, {"value": "1.5", "module": "A1-A3"}, {"value": "0.028", "module": "A4"}, {"value": "0.0579", "module": "A5"}, {"value": "0.00064", "module": "C1"}, {"value": "0.00223", "module": "C2"}, {"value": "0", "module": "C3", "scenario": "S2"}, {"value": "0.00193", "module": "C3", "scenario": "S3"}, {"value": "0.0152", "module": "C4"}, {"value": "-0.0512", "module": "D", "scenario": "S0"}, {"value": "-1.5", "module": "D", "scenario": "S2"}, {"value": "-0.143", "module": "D", "scenario": "S3"}]}}, {"referenceToLCIAMethodDataSet": {"shortDescription": [{"value": "Global Warming Potential biogenic (GWP-biogenic)", "lang": "en"}], "type": "LCIA method data set", "refObjectId": "2356e1ab-0185-4db5-86e5-16de51c7485c", "uri": "../lciamethods/2356e1ab-0185-4db5-86e5-16de51c7485c.xml"}, "other": {"anies": [{"name": "referenceToUnitGroupDataSet", "value": {"shortDescription": [{"value": "kg CO_(2)-Äq.", "lang": "en"}], "type": "unit group data set", "refObjectId": "1ebf3012-d0db-4de2-aefd-ef30cedb0be1", "uri": "../unitgroups/1ebf3012-d0db-4de2-aefd-ef30cedb0be1.xml"}}, {"value": "-0.0472", "module": "A1-A3"}, {"value": "0.00133", "module": "A4"}, {"value": "0.0653", "module": "A5"}, {"value": "1.93E-06", "module": "C1"}, {"value": "0.000106", "module": "C2"}, {"value": "0", "module": "C3", "scenario": "S2"}, {"value": "1.7E-05", "module": "C3", "scenario": "S3"}, {"value": "4.86E-05", "module": "C4"}, {"value": "-0.000117", "module": "D", "scenario": "S0"}, {"value": "0.0472", "module": "D", "scenario": "S2"}, {"value": "-0.000225", "module": "D", "scenario": "S3"}]}}, {"referenceToLCIAMethodDataSet": {"shortDescription": [{"value": "Global Warming Potential luluc (GWP-luluc)", "lang": "en"}], "type": "LCIA method data set", "refObjectId": "4331bbdb-978a-490d-8707-eeb047f01a55", "uri": "../lciamethods/4331bbdb-978a-490d-8707-eeb047f01a55.xml"}, "other": {"anies": [{"name": "referenceToUnitGroupDataSet", "value": {"shortDescription": [{"value": "kg CO_(2)-Äq.", "lang": "en"}], "type": "unit group data set", "refObjectId": "1ebf3012-d0db-4de2-aefd-ef30cedb0be1", "uri": "../unitgroups/1ebf3012-d0db-4de2-aefd-ef30cedb0be1.xml"}}, {"value": "0.000848", "module": "A1-A3"}, {"value": "0.000228", "module": "A4"}, {"value": "3.94E-06", "module": "A5"}, {"value": "4.99E-06", "module": "C1"}, {"value": "1.81E-05", "module": "C2"}, {"value": "0", "module": "C3", "scenario": "S2"}, {"value": "2.8E-06", "module": "C3", "scenario": "S3"}, {"value": "4.37E-05", "module": "C4"}, {"value": "-3.35E-05", "module": "D", "scenario": "S0"}, {"value": "-0.000848", "module": "D", "scenario": "S2"}, {"value": "-3.43E-05", "module": "D", "scenario": "S3"}]}}, {"referenceToLCIAMethodDataSet": {"shortDescription": [{"value": "Depletion potential of the stratospheric ozone layer (ODP)", "lang": "en"}], "type": "LCIA method data set", "refObjectId": "b5c629d6-def3-11e6-bf01-fe55135034f3", "uri": "../lciamethods/b5c629d6-def3-11e6-bf01-fe55135034f3.xml"}, "other": {"anies": [{"name": "referenceToUnitGroupDataSet", "value": {"shortDescription": [{"value": "kg CFC11-Äq.", "lang": "en"}], "type": "unit group data set", "refObjectId": "d9e957c9-7309-4474-bf3a-7777df6c4e5b", "uri": "../unitgroups/d9e957c9-7309-4474-bf3a-7777df6c4e5b.xml"}}, {"value": "1.01E-13", "module": "A1-A3"}, {"value": "3.38E-18", "module": "A4"}, {"value": "3.75E-17", "module": "A5"}, {"value": "7.41E-20", "module": "C1"}, {"value": "2.68E-19", "module": "C2"}, {"value": "0", "module": "C3", "scenario": "S2"}, {"value": "4.25E-17", "module": "C3", "scenario": "S3"}, {"value": "5.62E-17", "module": "C4"}, {"value": "-4.98E-16", "module": "D", "scenario": "S0"}, {"value": "-1.01E-13", "module": "D", "scenario": "S2"}, {"value": "-2.61E-16", "module": "D", "scenario": "S3"}]}}, {"referenceToLCIAMethodDataSet": {"shortDescription": [{"value": "Acidification potential of land and water (AP)", "lang": "en"}], "type": "LCIA method data set", "refObjectId": "b5c611c6-def3-11e6-bf01-fe55135034f3", "uri": "../lciamethods/b5c611c6-def3-11e6-bf01-fe55135034f3.xml"}, "other": {"anies": [{"name": "referenceToUnitGroupDataSet", "value": {"shortDescription": [{"value": "mol H^(+)-Äq.", "lang": "en"}], "type": "unit group data set", "refObjectId": "42e089ac-92bf-4bf2-8ca1-5fc40d18f2ed", "uri": "../unitgroups/42e089ac-92bf-4bf2-8ca1-5fc40d18f2ed.xml"}}, {"value": "0.00477", "module": "A1-A3"}, {"value": "2.95E-05", "module": "A4"}, {"value": "2.14E-05", "module": "A5"}, {"value": "3.09E-06", "module": "C1"}, {"value": "7.17E-06", "module": "C2"}, {"value": "0", "module": "C3", "scenario": "S2"}, {"value": "4.26E-06", "module": "C3", "scenario": "S3"}, {"value": "0.000109", "module": "C4"}, {"value": "-6.91E-05", "module": "D", "scenario": "S0"}, {"value": "-0.00477", "module": "D", "scenario": "S2"}, {"value": "-0.000132", "module": "D", "scenario": "S3"}]}}, {"referenceToLCIAMethodDataSet": {"shortDescription": [{"value": "Eutrophication potential aquatic freshwater (EP-freshwater)", "lang": "en"}], "type": "LCIA method data set", "refObjectId": "b53ec18f-7377-4ad3-86eb-cc3f4f276b2b", "uri": "../lciamethods/b53ec18f-7377-4ad3-86eb-cc3f4f276b2b.xml"}, "other": {"anies": [{"name": "referenceToUnitGroupDataSet", "value": {"shortDescription": [{"value": "kg PO_(4)-Äq.", "lang": "en"}], "type": "unit group data set", "refObjectId": "0429039d-a61d-4590-ba67-aa4a20a810a1", "uri": "../unitgroups/0429039d-a61d-4590-ba67-aa4a20a810a1.xml"}}, {"value": "2.73E-05", "module": "A1-A3"}, {"value": "8.55E-08", "module": "A4"}, {"value": "5.99E-09", "module": "A5"}, {"value": "1.87E-09", "module": "C1"}, {"value": "6.79E-09", "module": "C2"}, {"value": "0", "module": "C3", "scenario": "S2"}, {"value": "5.16E-09", "module": "C3", "scenario": "S3"}, {"value": "2.6E-08", "module": "C4"}, {"value": "-6.16E-08", "module": "D", "scenario": "S0"}, {"value": "-2.73E-05", "module": "D", "scenario": "S2"}, {"value": "-5.23E-08", "module": "D", "scenario": "S3"}]}}, {"referenceToLCIAMethodDataSet": {"shortDescription": [{"value": "Eutrophication potential aquatic marine (EP-marine)", "lang": "en"}], "type": "LCIA method data set", "refObjectId": "b5c619fa-def3-11e6-bf01-fe55135034f3", "uri": "../lciamethods/b5c619fa-def3-11e6-bf01-fe55135034f3.xml"}, "other": {"anies": [{"name": "referenceToUnitGroupDataSet", "value": {"shortDescription": [{"value": "kg N-Äq.", "lang": "en"}], "type": "unit group data set", "refObjectId": "d05bb823-ecdf-4686-8c40-bf1d9257859f", "uri": "../unitgroups/d05bb823-ecdf-4686-8c40-bf1d9257859f.xml"}}, {"value": "0.00179", "module": "A1-A3"}, {"value": "8.74E-06", "module": "A4"}, {"value": "6.07E-06", "module": "A5"}, {"value": "1.44E-06", "module": "C1"}, {"value": "3.23E-06", "module": "C2"}, {"value": "0", "module": "C3", "scenario": "S2"}, {"value": "9.47E-07", "module": "C3", "scenario": "S3"}, {"value": "2.8E-05", "module": "C4"}, {"value": "-1.81E-05", "module": "D", "scenario": "S0"}, {"value": "-0.00179", "module": "D", "scenario": "S2"}, {"value": "-4.75E-05", "module": "D", "scenario": "S3"}]}}, {"referenceToLCIAMethodDataSet": {"shortDescription": [{"value": "Eutrophication potential terrestrial (EP-terrestrial)", "lang": "en"}], "type": "LCIA method data set", "refObjectId": "b5c614d2-def3-11e6-bf01-fe55135034f3", "uri": "../lciamethods/b5c614d2-def3-11e6-bf01-fe55135034f3.xml"}, "other": {"anies": [{"name": "referenceToUnitGroupDataSet", "value": {"shortDescription": [{"value": "mol N-Äq.", "lang": "en"}], "type": "unit group data set", "refObjectId": "71b4d617-0ec9-4d3f-b65e-e438940c2401", "uri": "../unitgroups/71b4d617-0ec9-4d3f-b65e-e438940c2401.xml"}}, {"value": "0.0189", "module": "A1-A3"}, {"value": "0.000105", "module": "A4"}, {"value": "9.84E-05", "module": "A5"}, {"value": "1.59E-05", "module": "C1"}, {"value": "3.61E-05", "module": "C2"}, {"value": "0", "module": "C3", "scenario": "S2"}, {"value": "9.95E-06", "module": "C3", "scenario": "S3"}, {"value": "0.000308", "module": "C4"}, {"value": "-0.000195", "module": "D", "scenario": "S0"}, {"value": "-0.0189", "module": "D", "scenario": "S2"}, {"value": "-0.000523", "module": "D", "scenario": "S3"}]}}, {"referenceToLCIAMethodDataSet": {"shortDescription": [{"value": "Formation potential of tropospheric ozone photochemical oxidants (POCP)", "lang": "en"}], "type": "LCIA method data set", "refObjectId": "b5c610fe-def3-11e6-bf01-fe55135034f3", "uri": "../lciamethods/b5c610fe-def3-11e6-bf01-fe55135034f3.xml"}, "other": {"anies": [{"name": "referenceToUnitGroupDataSet", "value": {"shortDescription": [{"value": "kg NMVOC-Äq.", "lang": "en"}], "type": "unit group data set", "refObjectId": "d27c25f8-fbc1-44c6-b47b-4adbae4199c6", "uri": "../unitgroups/d27c25f8-fbc1-44c6-b47b-4adbae4199c6.xml"}}, {"value": "0.00413", "module": "A1-A3"}, {"value": "2.4E-05", "module": "A4"}, {"value": "1.65E-05", "module": "A5"}, {"value": "4.03E-06", "module": "C1"}, {"value": "6.33E-06", "module": "C2"}, {"value": "0", "module": "C3", "scenario": "S2"}, {"value": "2.59E-06", "module": "C3", "scenario": "S3"}, {"value": "8.48E-05", "module": "C4"}, {"value": "-5.23E-05", "module": "D", "scenario": "S0"}, {"value": "-0.00413", "module": "D", "scenario": "S2"}, {"value": "-0.000144", "module": "D", "scenario": "S3"}]}}, {"referenceToLCIAMethodDataSet": {"shortDescription": [{"value": "Abiotic depletion potential for non fossil resources (ADPE)", "lang": "en"}], "type": "LCIA method data set", "refObjectId": "b2ad6494-c78d-11e6-9d9d-cec0c932ce01", "uri": "../lciamethods/b2ad6494-c78d-11e6-9d9d-cec0c932ce01.xml"}, "other": {"anies": [{"name": "referenceToUnitGroupDataSet", "value": {"shortDescription": [{"value": "kg Sb-Äq.", "lang": "en"}], "type": "unit group data set", "refObjectId": "54ccd2d9-a32a-4fc2-923d-f2c8c93e89d4", "uri": "../unitgroups/54ccd2d9-a32a-4fc2-923d-f2c8c93e89d4.xml"}}, {"value": "2.38E-07", "module": "A1-A3"}, {"value": "2.02E-09", "module": "A4"}, {"value": "5.33E-10", "module": "A5"}, {"value": "4.42E-11", "module": "C1"}, {"value": "1.6E-10", "module": "C2"}, {"value": "0", "module": "C3", "scenario": "S2"}, {"value": "5.59E-10", "module": "C3", "scenario": "S3"}, {"value": "1.36E-09", "module": "C4"}, {"value": "-8E-09", "module": "D", "scenario": "S0"}, {"value": "-2.38E-07", "module": "D", "scenario": "S2"}, {"value": "-1.01E-08", "module": "D", "scenario": "S3"}]}}, {"referenceToLCIAMethodDataSet": {"shortDescription": [{"value": "Abiotic depletion potential for fossil resources (ADPF)", "lang": "en"}], "type": "LCIA method data set", "refObjectId": "b2ad6110-c78d-11e6-9d9d-cec0c932ce01", "uri": "../lciamethods/b2ad6110-c78d-11e6-9d9d-cec0c932ce01.xml"}, "other": {"anies": [{"name": "referenceToUnitGroupDataSet", "value": {"shortDescription": [{"value": "MJ", "lang": "en"}], "type": "unit group data set", "refObjectId": "93a60a57-a3c8-11da-a746-0800200c9a66", "uri": "../unitgroups/93a60a57-a3c8-11da-a746-0800200c9a66.xml"}}, {"value": "23", "module": "A1-A3"}, {"value": "0.374", "module": "A4"}, {"value": "0.0419", "module": "A5"}, {"value": "0.0082", "module": "C1"}, {"value": "0.0297", "module": "C2"}, {"value": "0", "module": "C3", "scenario": "S2"}, {"value": "0.0339", "module": "C3", "scenario": "S3"}, {"value": "0.199", "module": "C4"}, {"value": "-0.866", "module": "D", "scenario": "S0"}, {"value": "-23", "module": "D", "scenario": "S2"}, {"value": "-2.35", "module": "D", "scenario": "S3"}]}}, {"referenceToLCIAMethodDataSet": {"shortDescription": [{"value": "Water use (WDP)", "lang": "en"}], "type": "LCIA method data set", "refObjectId": "b2ad66ce-c78d-11e6-9d9d-cec0c932ce01", "uri": "../lciamethods/b2ad66ce-c78d-11e6-9d9d-cec0c932ce01.xml"}, "other": {"anies": [{"name": "referenceToUnitGroupDataSet", "value": {"shortDescription": [{"value": "m^(3) world-Äq. deprived", "lang": "en"}], "type": "unit group data set", "refObjectId": "6ae2df01-888e-46c8-b17d-49fa3869b476", "uri": "../unitgroups/6ae2df01-888e-46c8-b17d-49fa3869b476.xml"}}, {"value": "0.123", "module": "A1-A3"}, {"value": "0.000251", "module": "A4"}, {"value": "0.0129", "module": "A5"}, {"value": "5.51E-06", "module": "C1"}, {"value": "2E-05", "module": "C2"}, {"value": "0", "module": "C3", "scenario": "S2"}, {"value": "0.000421", "module": "C3", "scenario": "S3"}, {"value": "0.00159", "module": "C4"}, {"value": "-0.00494", "module": "D", "scenario": "S0"}, {"value": "-0.123", "module": "D", "scenario": "S2"}, {"value": "-0.00265", "module": "D", "scenario": "S3"}]}}, {"referenceToLCIAMethodDataSet": {"shortDescription": [{"value": "Incidence of disease due to PM emissions (PM)", "lang": "en"}], "type": "LCIA method data set", "refObjectId": "b5c602c6-def3-11e6-bf01-fe55135034f3", "uri": "../lciamethods/b5c602c6-def3-11e6-bf01-fe55135034f3.xml"}, "other": {"anies": [{"name": "referenceToUnitGroupDataSet", "value": {"shortDescription": [{"value": "Disease incidence", "lang": "en"}], "type": "unit group data set", "refObjectId": "3883559b-648f-4afc-8ba2-0bd24f3affa3", "uri": "../unitgroups/3883559b-648f-4afc-8ba2-0bd24f3affa3.xml"}}, {"value": "4.81E-08", "module": "A1-A3"}, {"value": "1.73E-10", "module": "A4"}, {"value": "1.88E-10", "module": "A5"}, {"value": "3.47E-11", "module": "C1"}, {"value": "3.92E-11", "module": "C2"}, {"value": "0", "module": "C3", "scenario": "S2"}, {"value": "3.58E-11", "module": "C3", "scenario": "S3"}, {"value": "1.35E-09", "module": "C4"}, {"value": "-5.88E-10", "module": "D", "scenario": "S0"}, {"value": "-4.81E-08", "module": "D", "scenario": "S2"}, {"value": "-7.1E-09", "module": "D", "scenario": "S3"}]}}, {"referenceToLCIAMethodDataSet": {"shortDescription": [{"value": "Human exposure efficiency relative to U235 (IR)", "lang": "en"}], "type": "LCIA method data set", "refObjectId": "b5c632be-def3-11e6-bf01-fe55135034f3", "uri": "../lciamethods/b5c632be-def3-11e6-bf01-fe55135034f3.xml"}, "other": {"anies": [{"name": "referenceToUnitGroupDataSet", "value": {"shortDescription": [{"value": "kBq U235-Äq.", "lang": "en"}], "type": "unit group data set", "refObjectId": "456b05bf-1415-44a9-9993-02452f554c09", "uri": "../unitgroups/456b05bf-1415-44a9-9993-02452f554c09.xml"}}, {"value": "0.0151", "module": "A1-A3"}, {"value": "6.71E-05", "module": "A4"}, {"value": "0.000225", "module": "A5"}, {"value": "1.47E-06", "module": "C1"}, {"value": "5.33E-06", "module": "C2"}, {"value": "0", "module": "C3", "scenario": "S2"}, {"value": "0.000845", "module": "C3", "scenario": "S3"}, {"value": "0.000232", "module": "C4"}, {"value": "-0.00989", "module": "D", "scenario": "S0"}, {"value": "-0.0151", "module": "D", "scenario": "S2"}, {"value": "-0.00513", "module": "D", "scenario": "S3"}]}}, {"referenceToLCIAMethodDataSet": {"shortDescription": [{"value": "Comparative toxic unit for ecosystems (ETP-fw)", "lang": "en"}], "type": "LCIA method data set", "refObjectId": "ee1082d1-b0f7-43ca-a1f0-21e2a4a74511", "uri": "../lciamethods/ee1082d1-b0f7-43ca-a1f0-21e2a4a74511.xml"}, "other": {"anies": [{"name": "referenceToUnitGroupDataSet", "value": {"shortDescription": [{"value": "CTUe", "lang": "en"}], "type": "unit group data set", "refObjectId": "aa959ded-f1eb-4efb-9c5c-2d60be36b3e6", "uri": "../unitgroups/aa959ded-f1eb-4efb-9c5c-2d60be36b3e6.xml"}}, {"value": "37.8", "module": "A1-A3"}, {"value": "0.265", "module": "A4"}, {"value": "0.0168", "module": "A5"}, {"value": "0.0058", "module": "C1"}, {"value": "0.021", "module": "C2"}, {"value": "0", "module": "C3", "scenario": "S2"}, {"value": "0.0145", "module": "C3", "scenario": "S3"}, {"value": "0.114", "module": "C4"}, {"value": "-0.175", "module": "D", "scenario": "S0"}, {"value": "-37.8", "module": "D", "scenario": "S2"}, {"value": "-0.129", "module": "D", "scenario": "S3"}]}}, {"referenceToLCIAMethodDataSet": {"shortDescription": [{"value": "Comparative toxic unit for humans (carcinogenic) (HTP-c)", "lang": "en"}], "type": "LCIA method data set", "refObjectId": "2299222a-bbd8-474f-9d4f-4dd1f18aea7c", "uri": "../lciamethods/2299222a-bbd8-474f-9d4f-4dd1f18aea7c.xml"}, "other": {"anies": [{"name": "referenceToUnitGroupDataSet", "value": {"shortDescription": [{"value": "CTUh", "lang": "en"}], "type": "unit group data set", "refObjectId": "d4c9523e-2d7e-49fd-8469-998f547d3a70", "uri": "../unitgroups/d4c9523e-2d7e-49fd-8469-998f547d3a70.xml"}}, {"value": "8.62E-10", "module": "A1-A3"}, {"value": "5.54E-12", "module": "A4"}, {"value": "1.29E-12", "module": "A5"}, {"value": "1.21E-13", "module": "C1"}, {"value": "4.4E-13", "module": "C2"}, {"value": "0", "module": "C3", "scenario": "S2"}, {"value": "4.01E-13", "module": "C3", "scenario": "S3"}, {"value": "1.68E-11", "module": "C4"}, {"value": "-7.96E-12", "module": "D", "scenario": "S0"}, {"value": "-8.62E-10", "module": "D", "scenario": "S2"}, {"value": "-1.76E-11", "module": "D", "scenario": "S3"}]}}, {"referenceToLCIAMethodDataSet": {"shortDescription": [{"value": "Comparative toxic unit for humans (noncarcinogenic) (HTP-nc)", "lang": "en"}], "type": "LCIA method data set", "refObjectId": "3af763a5-b7a1-48c9-9cee-1f223481fcef", "uri": "../lciamethods/3af763a5-b7a1-48c9-9cee-1f223481fcef.xml"}, "other": {"anies": [{"name": "referenceToUnitGroupDataSet", "value": {"shortDescription": [{"value": "CTUh", "lang": "en"}], "type": "unit group data set", "refObjectId": "d4c9523e-2d7e-49fd-8469-998f547d3a70", "uri": "../unitgroups/d4c9523e-2d7e-49fd-8469-998f547d3a70.xml"}}, {"value": "3.63E-08", "module": "A1-A3"}, {"value": "2.87E-10", "module": "A4"}, {"value": "1.03E-10", "module": "A5"}, {"value": "7.28E-12", "module": "C1"}, {"value": "2.58E-11", "module": "C2"}, {"value": "0", "module": "C3", "scenario": "S2"}, {"value": "1.48E-11", "module": "C3", "scenario": "S3"}, {"value": "1.86E-09", "module": "C4"}, {"value": "-2.96E-10", "module": "D", "scenario": "S0"}, {"value": "-3.63E-08", "module": "D", "scenario": "S2"}, {"value": "-6.73E-10", "module": "D", "scenario": "S3"}]}}, {"referenceToLCIAMethodDataSet": {"shortDescription": [{"value": "Soil quality index (SQP)", "lang": "en"}], "type": "LCIA method data set", "refObjectId": "b2ad6890-c78d-11e6-9d9d-cec0c932ce01", "uri": "../lciamethods/b2ad6890-c78d-11e6-9d9d-cec0c932ce01.xml"}, "other": {"anies": [{"name": "referenceToUnitGroupDataSet", "value": {"shortDescription": [{"value": "SQP", "lang": "en"}], "type": "unit group data set", "refObjectId": "f130951c-e67f-4f7f-8dd4-665de3974e18", "uri": "../unitgroups/f130951c-e67f-4f7f-8dd4-665de3974e18.xml"}}, {"value": "17.1", "module": "A1-A3"}, {"value": "0.131", "module": "A4"}, {"value": "0.0122", "module": "A5"}, {"value": "0.00288", "module": "C1"}, {"value": "0.0104", "module": "C2"}, {"value": "0", "module": "C3", "scenario": "S2"}, {"value": "0.0108", "module": "C3", "scenario": "S3"}, {"value": "0.0415", "module": "C4"}, {"value": "-0.127", "module": "D", "scenario": "S0"}, {"value": "-17.1", "module": "D", "scenario": "S2"}, {"value": "-0.0761", "module": "D", "scenario": "S3"}]}}]}, "otherAttributes": {"{http://www.indata.network/EPD/2019}epd-version": "1.2"}, "version": "1.1", "locations": "../ILCDLocations.xml"}