{"processInformation": {"dataSetInformation": {"UUID": "53b9dc3a-0128-40b9-b363-750bf86e342b", "name": {"baseName": [{"value": "Mehrschichtparkett (Parador GmbH)", "lang": "de"}, {"value": "Multi-layered engineered wood flooring (Parador GmbH)", "lang": "en"}], "functionalUnitFlowProperties": [{"lang": "de"}]}, "classificationInformation": {"classification": [{"class": [{"value": "Holz", "level": 0, "classId": "3"}, {"value": "Holzböden", "level": 1, "classId": "3.3"}, {"value": "Parkett", "level": 2, "classId": "3.3.02"}], "name": "OEKOBAU.DAT"}, {"class": [{"value": "02 Bauprodukte", "level": 0}, {"value": "Produkte aus Bauholz", "level": 1}, {"value": "Vollholzprodukte", "level": 2}], "name": "IBUCategories"}]}, "generalComment": [{"value": "Parador Mehrschichtparkettbden sind Holzfubden mit einer Edelholz-Deckschicht. Die fr die Herstellung dieser Bden bentigten Materialien wie Schnittholz, Hobelware, Friese, Furnier oder bereits fertige Deckschichten werden zunchst getrennt hergestellt. Hierfr kommen berwiegend heimische Holzarten zum Einsatz. Tropenhlzer werden aus kologischen Grnden nicht verwendet. Je nach Produktvariante besteht die Deckschicht aus einer einzelnen Lamelle oder aus mehreren Lamellen. Die einzelnen Materialien werden miteinander verleimt. Nach einer Klimatisierungszeit durchlaufen die Rohlinge eine Oberflchenbehandlung und werden entsprechend der Produktformate mit einem Lngs- und Querprofil versehen und verpackt.", "lang": "de"}, {"value": "Parador multi-layered engineered wood floors are wooden floors with a high-grade timber top layer. The materials required for the production of these floors, such as sawn timber, planed timber, friezes, veneers or ready-made top layers, are initially manufactured separately. For the most part, native wood species are used. Tropical woods are not used for environmental reasons. Depending on the version of the product, the top layer consists of either a single lamella or several lamellae. The individual materials are glued together. After a period of acclimatisation, the blanks undergo a surface treatment and are given a longitudinal and transverse profile according to the product format in question and are then packaged.", "lang": "en"}], "other": {"anies": [{"scenario": [{"description": [{"value": "Thermische Verwertung", "lang": "de"}, {"value": "Thermal recovery", "lang": "en"}], "name": "S1", "default": true}, {"description": [{"value": "Stoffliche Verwertung", "lang": "de"}, {"value": "Recycling of materials", "lang": "en"}], "name": "S2"}]}]}}, "quantitativeReference": {"referenceToReferenceFlow": [0]}, "time": {"referenceYear": 2023, "dataSetValidUntil": 2028, "other": {"anies": [{"name": "publicationDateOfEPD", "value": 1683158400000}]}}, "geography": {"locationOfOperationSupplyOrProduction": {"location": "RER"}}, "technology": {"technologyDescriptionAndIncludedProcesses": [{"value": "Nutzschicht, Mittellage und der Gegenzug werden in einem Arbeitsschritt in einer Presse unter Angabe eines Leims miteinander verpresst. Nach dem Verpressen werden die einzelnen Rohdielen einer Oberflächenbehandlung unterzogen (bis auf unbehandelte Endprodukte) und mit einem Längs- und Querprofil versehen. Nach der Qualitätskontrolle der einzelnen Mehrschichtparkettelemente werden diese in Halbschalen-Kartons abgepackt und in PE-Schrumpffolie verpackt. Diese einzelnen Verpackungseinheiten werden entsprechend der unterschiedlichen Formate auf Paletten gestapelt und im Lager für die nachfolgende Auslieferung bereitgestellt. Alle Prozesse werden im Rahmen der werkseigenen Factory Production Control (FPC) kontinuierlich überprüft und dokumentiert. Das Qualitätsmanagementsystem von Parador ist nach ISO 9001 zertifiziert und stellt sicher, dass alle Prozesse dokumentiert und bei Bedarf angepasst werden. \nTechnische Daten: \nWesentliche Merkmale und Leistung gem Leistungserklrung und zugrunde liegender harmonisierter Produktnorm EN 14342. \nDeklarierte Einheit: \nDie deklarierte Einheit ist 1 m durchschnittliches Mehrschichtparkett inkl. Verpackungsmaterialien. Der Durchschnitt wurde nach dem Produktionsvolumen der einbezogenen Produkte gewichtet. Es wurden die gesamten Inputs, Outputs sowie produzierten m2 fr den Betrachtungszeitraum zugrunde gelegt.\n\nDie im Durchschnitt enthaltenen Varianten unterscheiden sich in Bezug auf die Holzart und Behandlung der Nutzschicht sowie der Mae.", "lang": "de"}, {"value": "The wear layer, middle layer and backing are pressed together with glue in a press in one operation. After pressing, the individual raw planks undergo a surface treatment (apart from untreated end products) and are given a longitudinal and transverse profile. After quality control of the individual multi-layered engineered wood flooring elements, they are packed into half-shell cardboard boxes and shrink-wrapped in polyethylene (PE) film. These individual packaging units are stacked on pallets according to the different formats and made available in the warehouse for subsequent delivery. All processes are continually inspected and documented as part of the in-house Factory Production Control (FPC) system. Parador's quality management system is certified according to ISO 9001 and ensures that all processes are documented and, where necessary, amended. \nTechnical data: \nKey features and performance in accordance with the Declaration of Performance and the underlying harmonised product standard EN 14342. \nDeclared unit: \nThe declared unit is 1 m2 of average multi-layered engineered wood flooring, including packaging material. The average was weighted according to the production volume of the products involved. The total inputs, outputs and m2 produced for the period under consideration were taken as a basis. \n\nThe variations included on average differ in regard to the type of wood and the treatment of the wear layer and in terms of dimensions.", "lang": "en"}], "technologicalApplicability": [{"value": "Mehrschichtparkettbden sind Bodenbelge nach der EN 13489 fr eine private und gewerbliche Nutzung im Innenbereich, die entweder auf Estrich oder bestehenden anderen Unterbden wie Holz oder Fliesen in Verbindung mit geeigneten Verlegeunterlagen schwimmend verlegt oder aber vollflchig auf dem Estrich verklebt werden. Die Verlegung ist gem der den Paketen beiliegenden Verlegeanleitung bzw. dem \"Ratgeber Parkett\", den Regeln des Fachs und dem Stand der Technik durchzufhren.\nFr die Verwendung gelten die jeweiligen nationalen Bestimmungen.", "lang": "de"}, {"value": "Multi-layered engineered wood floors are floor coverings in accordance with EN 13489 for private and commercial use in interior areas, which are either laid \"floating\" on screed or on other existing floors such as wood or tiles, in connection with suitable underlay materials, or are glued to the screed across the whole floor area. Laying is to be done in accordance with the laying instructions in the packaging or the \"Guide Engineered Wood Flooring\", the rules of the trade and using the latest methods in terms of technology. The respective national regulations apply to the use of the product.", "lang": "en"}]}}, "modellingAndValidation": {"LCIMethodAndAllocation": {"typeOfDataSet": "EPD", "referenceToLCAMethodDetails": [{"shortDescription": [{"value": "Vollholzprodukte.pdf", "lang": "de"}], "type": "source data set", "refObjectId": "f8246994-3590-473c-8f25-87df8f61a5c4"}], "other": {"anies": [{"name": "subType", "value": "average dataset"}]}}, "dataSourcesTreatmentAndRepresentativeness": {"referenceToDataSource": [{"shortDescription": [{"value": "GaBi Database (all versions)", "lang": "de"}], "type": "source data set", "refObjectId": "28d74cc0-db8b-4d7e-bc44-5f6d56ce0c4a"}, {"shortDescription": [{"value": "GaBi Database Edition 2021, CUP 2021.01", "lang": "de"}], "type": "source data set", "refObjectId": "1cece811-7501-44d4-8067-9259bd5cb835"}], "useAdviceForDataSet": [{"value": "Gültigkeitsbereich: \nDie vorliegende EPD bezieht sich auf Herstellung, Transport, Installation und Entsorgung eines durchschnittlichen Quadratmeters Mehrschichtparkett von Parador. Die technischen Eigenschaften werden in Kapitel 2.3 dargestellt. Produktionsstandort des Produkts ist Gssing in sterreich. Der Versand erfolgt vom Standort Coesfeld in Deutschland. \nSystemgrenze: \nTyp der EPD: Wiege bis Werkstor mit Optionen.\n\nModule A1–A3 und A5\nIn den Modulen A1–A3 wird die Produktion der notwendigen Rohstoffe und Energien inklusive aller entsprechenden Vorketten sowie der Beschaffungstransporte bercksichtigt.\nAuerdem wird die gesamte Herstellungsphase inklusive der Behandlung von Produktionsabfllen bis zum Erreichen des End-of-Waste-Status (EoW) betrachtet.\nIn Modul A5 wird die Verwertung der Verpackungsmaterialien bilanziert.\n\nModule B2 und B5\nIn Modul B2 wird die Reinigung und das len des Parketts einschlielich der dafr bentigten Hilfsstoffe sowie die Behandlung der dabei anfallenden Abflle und Abwasser in der Referenznutzungsdauer betrachtet.\nIn Modul B5 wird die Renovierung des Parketts einschlielich der Behandlung der dabei anfallenden Abflle deklariert.\n\nModule C1–C4 und D\nModul C1 beschreibt den Rckbau. Da ein manueller Rckbau angenommen wird, werden in diesem Modul keine Lasten/Nutzen bilanziert.\nIm Modul C2 werden die Transporte zu den Entsorgungsprozessen betrachtet.\nDas Modul C3 beinhaltet die notwendigen Prozesse fr die Abfallbehandlung am Ende des Produktlebenswegs. Hierfr werden zwei Szenarien betrachtet: Thermische Verwertung (Szenario 1) und stoffliche Verwertung (Szenario 2).\n\nDie Lasten fr die Abfallbehandlung werden hierin so weit abgebildet, bis das Ende der Abfalleigenschaft erreicht ist. Dabei entstehende Potenziale und vermiedene Lasten auerhalb der Systemgrenze werden Modul D zugeordnet.\nEs werden keine Stoffe deponiert, sodass in Modul C4 keine Lasten/Nutzen bilanziert werden.", "lang": "de"}, {"value": "Scope: \nThis EPD relates to the manufacture, transport, installation, and disposal of an average square metre of Parador multi-layered engineered wood flooring. The technical characteristics are described in chapter 2.3. The product is manufactured in Gssing, Austria. It is shipped from Coesfeld in Germany. \nSystem boundary: \nType of EPD: Cradle to factory gate with options. \n\nModules A1 to A3 and A5 \nIn Modules A1 to A3, the production of the required raw materials and energy (including all relevant upstream chains and procurement transport) is taken into account. Furthermore, the entire manufacturing phase is considered, including treatment of production waste until end-of-waste status (EoW) is reached. In Module A5, the recovery of the packaging material is accounted for. \n\nModules B2 and B5 \nIn Module B2, the cleaning and oiling of the engineered wood flooring is considered, including the auxiliary materials needed for this and the treatment of the waste and waste water that is produced, in the referenced useful life. In Module B5, the renovation of the engineered wood flooring is declared, including the treatment of the waste that arises. \n\nModules C1 to C4 and D \nModule C1 describes the dismantling of the product. As it is assumed that dismantling will be done manually, no negative or positive effect is accounted for in this module. In Module C2, transportation to the various sites for disposal processes is taken into account. Module C2 comprises the necessary processes for waste management at the end of the product lifecycle. For this purpose, two scenarios are considered: thermal recovery (scenario 1) and recycling of materials (scenario 2). \n\nThe negative effects for waste management are mapped out here up until the point when the material loses its waste status. Potentials that arise and negative effects that are avoided outside of the system boundaries are assigned to Module D. No materials are sent to landfill so no negative or positive effects are accounted for in Module C4.", "lang": "en"}], "other": {"anies": [{"name": "referenceToOriginalEPD", "value": {"shortDescription": {"value": "Mehrschichtparkett.pdf", "defaultValue": "Mehrschichtparkett.pdf", "lstrings": [{"lang": "de", "value": "Mehrschichtparkett.pdf"}]}, "type": "source data set", "uuid": {"uuid": "ee2a70ef-d20f-4c37-b748-1a3955d0f8d9"}, "refObjectId": "ee2a70ef-d20f-4c37-b748-1a3955d0f8d9", "resourceURLs": ["https://oekobaudat.de/OEKOBAU.DAT/resource/sources/ee2a70ef-d20f-4c37-b748-1a3955d0f8d9/Mehrschichtparkett_18822.pdf?version=00.02.000"]}}]}}, "validation": {"review": [{"referenceToNameOfReviewerAndInstitution": [{"shortDescription": [{"value": "Institut Bauen und Umwelt e. V.", "lang": "de"}], "type": "contact data set", "refObjectId": "d111dbec-b024-4be5-86c5-752d6eb2cf95", "uri": "../contacts/d111dbec-b024-4be5-86c5-752d6eb2cf95.xml"}], "type": "Accredited third party review"}]}, "complianceDeclarations": {"compliance": [{"referenceToComplianceSystem": {"shortDescription": [{"value": "DIN EN 15804+A2", "lang": "de"}], "type": "source data set", "refObjectId": "c0016b33-8cf7-415c-ac6e-deba0d21440d", "uri": "../sources/c0016b33-8cf7-415c-ac6e-deba0d21440d.xml"}}, {"referenceToComplianceSystem": {"shortDescription": [{"value": "ISO 14025", "lang": "de"}], "type": "source data set", "refObjectId": "4f2eb655-6e44-4874-a95a-e28f5442cd4d", "uri": "../sources/4f2eb655-6e44-4874-a95a-e28f5442cd4d.xml"}}]}}, "administrativeInformation": {"commissionerAndGoal": {"referenceToCommissioner": [{"shortDescription": [{"value": "Parador GmbH", "lang": "de"}], "type": "contact data set", "refObjectId": "0861a318-be95-448b-b08e-751d226e2c2c", "uri": "../contacts/0861a318-be95-448b-b08e-751d226e2c2c.xml"}]}, "dataGenerator": {"referenceToPersonOrEntityGeneratingTheDataSet": [{"shortDescription": [{"value": "brands and values GmbH", "lang": "de"}], "type": "contact data set", "refObjectId": "6b539b8a-10e3-4004-8ccc-a79f169aa339", "uri": "../contacts/6b539b8a-10e3-4004-8ccc-a79f169aa339.xml"}]}, "dataEntryBy": {"timeStamp": 1683158400000, "referenceToDataSetFormat": [{"shortDescription": [{"value": "ILCD Format", "lang": "de"}], "type": "source data set", "refObjectId": "a97a0155-0234-4b87-b4ce-a45da52f2a40", "uri": "../sources/a97a0155-0234-4b87-b4ce-a45da52f2a40.xml"}, {"shortDescription": [{"value": "EPD-Datenformaterweiterungen v1.2", "lang": "de"}, {"value": "EPD Data Format Extensions v1.2", "lang": "en"}], "type": "source data set", "refObjectId": "a29449fd-aa2f-4de8-b5d7-4b06b43c6fde", "uri": "../sources/a29449fd-aa2f-4de8-b5d7-4b06b43c6fde.xml"}]}, "publicationAndOwnership": {"dataSetVersion": "00.13.000", "dateOfLastRevision": 1683193320000, "referenceToRegistrationAuthority": {"shortDescription": [{"value": "Institut Bauen und Umwelt e. V.", "lang": "de"}], "type": "contact data set", "refObjectId": "d111dbec-b024-4be5-86c5-752d6eb2cf95", "uri": "../contacts/d111dbec-b024-4be5-86c5-752d6eb2cf95.xml"}, "registrationNumber": "EPD-PAR-20230067-IBC1-DE", "referenceToOwnershipOfDataSet": {"shortDescription": [{"value": "Parador GmbH", "lang": "de"}], "type": "contact data set", "refObjectId": "0861a318-be95-448b-b08e-751d226e2c2c", "uri": "../contacts/0861a318-be95-448b-b08e-751d226e2c2c.xml"}, "copyright": true, "licenseType": "Free of charge for all users and uses", "accessRestrictions": [{"value": "None", "lang": "en"}], "other": {"anies": [{"name": "referenceToPublisher", "value": {"shortDescription": [{"value": "Institut Bauen und Umwelt e. V.", "lang": "de"}], "type": "contact data set", "refObjectId": "d111dbec-b024-4be5-86c5-752d6eb2cf95", "uri": "../contacts/d111dbec-b024-4be5-86c5-752d6eb2cf95.xml"}}]}}}, "exchanges": {"exchange": [{"dataSetInternalID": 0, "referenceToFlowDataSet": {"shortDescription": [{"value": "Mehrschichtparkett (Mehrschichtparkett)", "lang": "de"}], "type": "flow data set", "refObjectId": "4aef137d-5891-955e-4793-b5630b6d2f81", "uri": "../flows/4aef137d-5891-955e-4793-b5630b6d2f81.xml"}, "meanAmount": 1.0, "referencesToDataSource": {}, "referenceFlow": true, "resolvedFlowVersion": "00.03.000", "resultingflowAmount": 1.0, "flowProperties": [{"name": [{"lang": "de", "value": "Masse"}, {"lang": "en", "value": "Mass"}], "uuid": "93a60a56-a3c8-11da-a746-0800200b9a66", "meanValue": 7.01}, {"name": [{"lang": "de", "value": "Fläche"}, {"lang": "en", "value": "Area"}], "uuid": "93a60a56-a3c8-19da-a746-0800200c9a66", "referenceFlowProperty": true, "meanValue": 1.0, "referenceUnit": "qm", "unitGroupUUID": "c20a03d7-bd90-4569-bc94-66cfd364dfc8"}, {"name": [{"lang": "de", "value": "biogener Kohlenstoffgehalt in der Verpackung"}, {"lang": "en", "value": "Carbon content (biogenic) - packaging"}], "uuid": "262a541b-209e-44cc-a426-33bce30de7b1", "meanValue": 0.16}, {"name": [{"lang": "de", "value": "biogener Kohlenstoffgehalt"}, {"lang": "en", "value": "Carbon content (biogenic)"}], "uuid": "62e503ce-544a-4599-b2ad-bcea15a7bf20", "meanValue": 3.15}], "materialProperties": [{"name": "gross density", "value": "539.0", "unit": "kg/m^3", "unitDescription": "kilograms per cubic metre"}, {"name": "layer thickness", "value": "0.013", "unit": "m", "unitDescription": "meters"}, {"name": "grammage", "value": "7.01", "unit": "kg/m^2", "unitDescription": "kilograms per square meter"}], "typeOfFlow": "Product flow", "classification": {"classHierarchy": "Holz / Holzböden / Parkett", "name": "OEKOBAU.DAT"}}, {"dataSetInternalID": 1, "referenceToFlowDataSet": {"shortDescription": [{"value": "Erneuerbare Primärenergie als Energieträger (PERE)", "lang": "de"}, {"value": "Renewable primary energy as energy carrier (PERE)", "lang": "en"}], "type": "flow data set", "refObjectId": "20f32be5-0398-4288-9b6d-accddd195317", "uri": "../flows/20f32be5-0398-4288-9b6d-accddd195317.xml"}, "exchange direction": "INPUT", "other": {"anies": [{"name": "referenceToUnitGroupDataSet", "value": {"shortDescription": [{"value": "MJ", "lang": "de"}], "type": "unit group data set", "refObjectId": "93a60a57-a3c8-11da-a746-0800200c9a66", "uri": "../unitgroups/93a60a57-a3c8-11da-a746-0800200c9a66.xml"}}, {"value": "164.585604707085", "module": "A1-A3"}, {"value": "0.01281", "module": "A5"}, {"value": "51.8", "module": "B2"}, {"value": "5.592", "module": "B5"}, {"value": "0", "module": "C1"}, {"value": "0.05588", "module": "C2"}, {"value": "110.849843283343", "module": "C3", "scenario": "S1"}, {"value": "0.1864", "module": "C3", "scenario": "S2"}, {"value": "0", "module": "C4"}, {"value": "-18.16", "module": "D", "scenario": "S1"}, {"value": "-28.1", "module": "D", "scenario": "S2"}]}, "resolvedFlowVersion": "38.00.000", "flowProperties": [], "typeOfFlow": "Other flow", "classification": {"classHierarchy": "Quantities", "name": "GaBiCategories"}}, {"dataSetInternalID": 2, "referenceToFlowDataSet": {"shortDescription": [{"value": "Erneuerbare Primärenergie zur stofflichen Nutzung (PERM)", "lang": "de"}, {"value": "Renewable primary energy resources as material utilization (PERM)", "lang": "en"}], "type": "flow data set", "refObjectId": "fb3ec0de-548d-4508-aea5-00b73bf6f702", "uri": "../flows/fb3ec0de-548d-4508-aea5-00b73bf6f702.xml"}, "exchange direction": "INPUT", "other": {"anies": [{"name": "referenceToUnitGroupDataSet", "value": {"shortDescription": [{"value": "MJ", "lang": "de"}], "type": "unit group data set", "refObjectId": "93a60a57-a3c8-11da-a746-0800200c9a66", "uri": "../unitgroups/93a60a57-a3c8-11da-a746-0800200c9a66.xml"}}, {"value": "116.914395292915", "module": "A1-A3"}, {"value": "0", "module": "A5"}, {"value": "0", "module": "B2"}, {"value": "0", "module": "B5"}, {"value": "0", "module": "C1"}, {"value": "0", "module": "C2"}, {"value": "-110.371643283343", "module": "C3", "scenario": "S1"}, {"value": "0", "module": "C3", "scenario": "S2"}, {"value": "0", "module": "C4"}, {"value": "0", "module": "D", "scenario": "S1"}, {"value": "0", "module": "D", "scenario": "S2"}]}, "resolvedFlowVersion": "38.00.000", "flowProperties": [], "typeOfFlow": "Other flow", "classification": {"classHierarchy": "Quantities", "name": "GaBiCategories"}}, {"dataSetInternalID": 3, "referenceToFlowDataSet": {"shortDescription": [{"value": "Total erneuerbare Primärenergie (PERT)", "lang": "de"}, {"value": "Total use of renewable primary energy resources (PERT)", "lang": "en"}], "type": "flow data set", "refObjectId": "53f97275-fa8a-4cdd-9024-65936002acd0", "uri": "../flows/53f97275-fa8a-4cdd-9024-65936002acd0.xml"}, "exchange direction": "INPUT", "other": {"anies": [{"name": "referenceToUnitGroupDataSet", "value": {"shortDescription": [{"value": "MJ", "lang": "de"}], "type": "unit group data set", "refObjectId": "93a60a57-a3c8-11da-a746-0800200c9a66", "uri": "../unitgroups/93a60a57-a3c8-11da-a746-0800200c9a66.xml"}}, {"value": "281.5", "module": "A1-A3"}, {"value": "0.01281", "module": "A5"}, {"value": "51.8", "module": "B2"}, {"value": "5.592", "module": "B5"}, {"value": "0", "module": "C1"}, {"value": "0.05588", "module": "C2"}, {"value": "0.4782", "module": "C3", "scenario": "S1"}, {"value": "0.1864", "module": "C3", "scenario": "S2"}, {"value": "0", "module": "C4"}, {"value": "-18.16", "module": "D", "scenario": "S1"}, {"value": "-28.1", "module": "D", "scenario": "S2"}]}, "resolvedFlowVersion": "38.00.000", "flowProperties": [], "typeOfFlow": "Other flow", "classification": {"classHierarchy": "Quantities / Environmental quantities / EPD EN 15804 / LCI indicators", "name": "GaBiCategories"}}, {"dataSetInternalID": 4, "referenceToFlowDataSet": {"shortDescription": [{"value": "Nicht-erneuerbare Primärenergie als Energieträger (PENRE)", "lang": "de"}, {"value": "Non renewable primary energy as energy carrier (PENRE)", "lang": "en"}], "type": "flow data set", "refObjectId": "ac857178-2b45-46ec-892a-a9a4332f0372", "uri": "../flows/ac857178-2b45-46ec-892a-a9a4332f0372.xml"}, "exchange direction": "INPUT", "other": {"anies": [{"name": "referenceToUnitGroupDataSet", "value": {"shortDescription": [{"value": "MJ", "lang": "de"}], "type": "unit group data set", "refObjectId": "93a60a57-a3c8-11da-a746-0800200c9a66", "uri": "../unitgroups/93a60a57-a3c8-11da-a746-0800200c9a66.xml"}}, {"value": "80.6804834044512", "module": "A1-A3"}, {"value": "0.0933", "module": "A5"}, {"value": "127.9", "module": "B2"}, {"value": "26.41", "module": "B5"}, {"value": "0", "module": "C1"}, {"value": "0.9746", "module": "C2"}, {"value": "8.48548142554599", "module": "C3", "scenario": "S1"}, {"value": "1.264", "module": "C3", "scenario": "S2"}, {"value": "0", "module": "C4"}, {"value": "-80.01", "module": "D", "scenario": "S1"}, {"value": "-3.014", "module": "D", "scenario": "S2"}]}, "resolvedFlowVersion": "38.00.000", "flowProperties": [], "typeOfFlow": "Other flow", "classification": {"classHierarchy": "Quantities", "name": "GaBiCategories"}}, {"dataSetInternalID": 5, "referenceToFlowDataSet": {"shortDescription": [{"value": "Nicht-erneuerbare Primärenergie zur stofflichen Nutzung (PENRM)", "lang": "de"}, {"value": "Non renewable primary energy as material utilization (PENRM)", "lang": "en"}], "type": "flow data set", "refObjectId": "1421caa0-679d-4bf4-b282-0eb850ccae27", "uri": "../flows/1421caa0-679d-4bf4-b282-0eb850ccae27.xml"}, "exchange direction": "INPUT", "other": {"anies": [{"name": "referenceToUnitGroupDataSet", "value": {"shortDescription": [{"value": "MJ", "lang": "de"}], "type": "unit group data set", "refObjectId": "93a60a57-a3c8-11da-a746-0800200c9a66", "uri": "../unitgroups/93a60a57-a3c8-11da-a746-0800200c9a66.xml"}}, {"value": "10.8595165955488", "module": "A1-A3"}, {"value": "0", "module": "A5"}, {"value": "0", "module": "B2"}, {"value": "0", "module": "B5"}, {"value": "0", "module": "C1"}, {"value": "0", "module": "C2"}, {"value": "-6.01848142554599", "module": "C3", "scenario": "S1"}, {"value": "0", "module": "C3", "scenario": "S2"}, {"value": "0", "module": "C4"}, {"value": "0", "module": "D", "scenario": "S1"}, {"value": "0", "module": "D", "scenario": "S2"}]}, "resolvedFlowVersion": "38.00.000", "flowProperties": [], "typeOfFlow": "Other flow", "classification": {"classHierarchy": "Quantities", "name": "GaBiCategories"}}, {"dataSetInternalID": 6, "referenceToFlowDataSet": {"shortDescription": [{"value": "Total nicht erneuerbare Primärenergie (PENRT)", "lang": "de"}, {"value": "Total use of non renewable primary energy resources (PENRT)", "lang": "en"}], "type": "flow data set", "refObjectId": "06159210-646b-4c8d-8583-da9b3b95a6c1", "uri": "../flows/06159210-646b-4c8d-8583-da9b3b95a6c1.xml"}, "exchange direction": "INPUT", "other": {"anies": [{"name": "referenceToUnitGroupDataSet", "value": {"shortDescription": [{"value": "MJ", "lang": "de"}], "type": "unit group data set", "refObjectId": "93a60a57-a3c8-11da-a746-0800200c9a66", "uri": "../unitgroups/93a60a57-a3c8-11da-a746-0800200c9a66.xml"}}, {"value": "91.54", "module": "A1-A3"}, {"value": "0.0933", "module": "A5"}, {"value": "127.9", "module": "B2"}, {"value": "26.41", "module": "B5"}, {"value": "0", "module": "C1"}, {"value": "0.9746", "module": "C2"}, {"value": "2.467", "module": "C3", "scenario": "S1"}, {"value": "1.264", "module": "C3", "scenario": "S2"}, {"value": "0", "module": "C4"}, {"value": "-80.01", "module": "D", "scenario": "S1"}, {"value": "-3.014", "module": "D", "scenario": "S2"}]}, "resolvedFlowVersion": "38.00.000", "flowProperties": [], "typeOfFlow": "Other flow", "classification": {"classHierarchy": "Quantities / Environmental quantities / EPD EN 15804 / LCI indicators", "name": "GaBiCategories"}}, {"dataSetInternalID": 7, "referenceToFlowDataSet": {"shortDescription": [{"value": "Einsatz von Sekundärstoffen (SM)", "lang": "de"}, {"value": "Use of secondary material (SM)", "lang": "en"}], "type": "flow data set", "refObjectId": "c6a1f35f-2d09-4f54-8dfb-97e502e1ce92", "uri": "../flows/c6a1f35f-2d09-4f54-8dfb-97e502e1ce92.xml"}, "exchange direction": "INPUT", "other": {"anies": [{"name": "referenceToUnitGroupDataSet", "value": {"shortDescription": [{"value": "kg", "lang": "de"}], "type": "unit group data set", "refObjectId": "ad38d542-3fe9-439d-9b95-2f5f7752acaf", "uri": "../unitgroups/ad38d542-3fe9-439d-9b95-2f5f7752acaf.xml"}}, {"value": "0", "module": "A1-A3"}, {"value": "0", "module": "A5"}, {"value": "0", "module": "B2"}, {"value": "0", "module": "B5"}, {"value": "0", "module": "C1"}, {"value": "0", "module": "C2"}, {"value": "0", "module": "C3", "scenario": "S1"}, {"value": "0", "module": "C3", "scenario": "S2"}, {"value": "0", "module": "C4"}, {"value": "0", "module": "D", "scenario": "S1"}, {"value": "0", "module": "D", "scenario": "S2"}]}, "resolvedFlowVersion": "38.00.000", "flowProperties": [], "typeOfFlow": "Other flow", "classification": {"classHierarchy": "Quantities / Environmental quantities / EPD EN 15804 / LCI indicators", "name": "GaBiCategories"}}, {"dataSetInternalID": 8, "referenceToFlowDataSet": {"shortDescription": [{"value": "Erneuerbare Sekundärbrennstoffe (RSF)", "lang": "de"}, {"value": "Use of renewable secondary fuels (RSF)", "lang": "en"}], "type": "flow data set", "refObjectId": "64333088-a55f-4aa2-9a31-c10b07816787", "uri": "../flows/64333088-a55f-4aa2-9a31-c10b07816787.xml"}, "exchange direction": "INPUT", "other": {"anies": [{"name": "referenceToUnitGroupDataSet", "value": {"shortDescription": [{"value": "MJ", "lang": "de"}], "type": "unit group data set", "refObjectId": "93a60a57-a3c8-11da-a746-0800200c9a66", "uri": "../unitgroups/93a60a57-a3c8-11da-a746-0800200c9a66.xml"}}, {"value": "0", "module": "A1-A3"}, {"value": "0", "module": "A5"}, {"value": "0", "module": "B2"}, {"value": "0", "module": "B5"}, {"value": "0", "module": "C1"}, {"value": "0", "module": "C2"}, {"value": "0", "module": "C3", "scenario": "S1"}, {"value": "0", "module": "C3", "scenario": "S2"}, {"value": "0", "module": "C4"}, {"value": "110.371643283343", "module": "D", "scenario": "S1"}, {"value": "0", "module": "D", "scenario": "S2"}]}, "resolvedFlowVersion": "38.00.000", "flowProperties": [], "typeOfFlow": "Other flow", "classification": {"classHierarchy": "Quantities / Environmental quantities / EPD EN 15804 / LCI indicators", "name": "GaBiCategories"}}, {"dataSetInternalID": 9, "referenceToFlowDataSet": {"shortDescription": [{"value": "Nicht erneuerbare Sekundärbrennstoffe (NRSF)", "lang": "de"}, {"value": "Use of non renewable secondary fuels (NRSF)", "lang": "en"}], "type": "flow data set", "refObjectId": "89def144-d39a-4287-b86f-efde453ddcb2", "uri": "../flows/89def144-d39a-4287-b86f-efde453ddcb2.xml"}, "exchange direction": "INPUT", "other": {"anies": [{"name": "referenceToUnitGroupDataSet", "value": {"shortDescription": [{"value": "MJ", "lang": "de"}], "type": "unit group data set", "refObjectId": "93a60a57-a3c8-11da-a746-0800200c9a66", "uri": "../unitgroups/93a60a57-a3c8-11da-a746-0800200c9a66.xml"}}, {"value": "0", "module": "A1-A3"}, {"value": "0", "module": "A5"}, {"value": "0", "module": "B2"}, {"value": "0", "module": "B5"}, {"value": "0", "module": "C1"}, {"value": "0", "module": "C2"}, {"value": "0", "module": "C3", "scenario": "S1"}, {"value": "0", "module": "C3", "scenario": "S2"}, {"value": "0", "module": "C4"}, {"value": "0", "module": "D", "scenario": "S1"}, {"value": "0", "module": "D", "scenario": "S2"}]}, "resolvedFlowVersion": "38.00.000", "flowProperties": [], "typeOfFlow": "Other flow", "classification": {"classHierarchy": "Quantities / Environmental quantities / EPD EN 15804 / LCI indicators", "name": "GaBiCategories"}}, {"dataSetInternalID": 10, "referenceToFlowDataSet": {"shortDescription": [{"value": "Einsatz von Süßwasserressourcen (FW)", "lang": "de"}, {"value": "Use of net fresh water (FW)", "lang": "en"}], "type": "flow data set", "refObjectId": "3cf952c8-f3a4-461d-8c96-96456ca62246", "uri": "../flows/3cf952c8-f3a4-461d-8c96-96456ca62246.xml"}, "exchange direction": "INPUT", "other": {"anies": [{"name": "referenceToUnitGroupDataSet", "value": {"shortDescription": [{"value": "m^3", "lang": "de"}], "type": "unit group data set", "refObjectId": "cd950537-0a98-4044-9ba7-9f9a68d0a504", "uri": "../unitgroups/cd950537-0a98-4044-9ba7-9f9a68d0a504.xml"}}, {"value": "0.07481", "module": "A1-A3"}, {"value": "0.0008811", "module": "A5"}, {"value": "0.05321", "module": "B2"}, {"value": "0.01283", "module": "B5"}, {"value": "0", "module": "C1"}, {"value": "6.4E-05", "module": "C2"}, {"value": "0.02758", "module": "C3", "scenario": "S1"}, {"value": "0.0009277", "module": "C3", "scenario": "S2"}, {"value": "0", "module": "C4"}, {"value": "-0.01774", "module": "D", "scenario": "S1"}, {"value": "-0.001164", "module": "D", "scenario": "S2"}]}, "resolvedFlowVersion": "38.00.000", "flowProperties": [], "typeOfFlow": "Other flow", "classification": {"classHierarchy": "Quantities / Environmental quantities / EPD EN 15804 / LCI indicators", "name": "GaBiCategories"}}, {"dataSetInternalID": 11, "referenceToFlowDataSet": {"shortDescription": [{"value": "Gefährlicher Abfall zur Deponie (HWD)", "lang": "de"}, {"value": "Hazardous waste disposed (HWD)", "lang": "en"}], "type": "flow data set", "refObjectId": "430f9e0f-59b2-46a0-8e0d-55e0e84948fc", "uri": "../flows/430f9e0f-59b2-46a0-8e0d-55e0e84948fc.xml"}, "exchange direction": "OUTPUT", "other": {"anies": [{"name": "referenceToUnitGroupDataSet", "value": {"shortDescription": [{"value": "kg", "lang": "de"}], "type": "unit group data set", "refObjectId": "ad38d542-3fe9-439d-9b95-2f5f7752acaf", "uri": "../unitgroups/ad38d542-3fe9-439d-9b95-2f5f7752acaf.xml"}}, {"value": "5.545E-07", "module": "A1-A3"}, {"value": "1.165E-11", "module": "A5"}, {"value": "3.056E-08", "module": "B2"}, {"value": "5.295E-09", "module": "B5"}, {"value": "0", "module": "C1"}, {"value": "5.135E-11", "module": "C2"}, {"value": "4.451E-10", "module": "C3", "scenario": "S1"}, {"value": "0", "module": "C3", "scenario": "S2"}, {"value": "0", "module": "C4"}, {"value": "-1.799E-08", "module": "D", "scenario": "S1"}, {"value": "0", "module": "D", "scenario": "S2"}]}, "resolvedFlowVersion": "38.00.000", "flowProperties": [], "typeOfFlow": "Other flow", "classification": {"classHierarchy": "Quantities / Environmental quantities / EPD EN 15804 / LCI indicators", "name": "GaBiCategories"}}, {"dataSetInternalID": 12, "referenceToFlowDataSet": {"shortDescription": [{"value": "Entsorgter nicht gefährlicher Abfall (NHWD)", "lang": "de"}, {"value": "Non hazardous waste disposed (NHWD)", "lang": "en"}], "type": "flow data set", "refObjectId": "b29ef66b-e286-4afa-949f-62f1a7b4d7fa", "uri": "../flows/b29ef66b-e286-4afa-949f-62f1a7b4d7fa.xml"}, "exchange direction": "OUTPUT", "other": {"anies": [{"name": "referenceToUnitGroupDataSet", "value": {"shortDescription": [{"value": "kg", "lang": "de"}], "type": "unit group data set", "refObjectId": "ad38d542-3fe9-439d-9b95-2f5f7752acaf", "uri": "../unitgroups/ad38d542-3fe9-439d-9b95-2f5f7752acaf.xml"}}, {"value": "0.1003", "module": "A1-A3"}, {"value": "0.001747", "module": "A5"}, {"value": "0.3403", "module": "B2"}, {"value": "0.03741", "module": "B5"}, {"value": "0", "module": "C1"}, {"value": "0.0001529", "module": "C2"}, {"value": "0.08144", "module": "C3", "scenario": "S1"}, {"value": "0", "module": "C3", "scenario": "S2"}, {"value": "0", "module": "C4"}, {"value": "-0.03763", "module": "D", "scenario": "S1"}, {"value": "0", "module": "D", "scenario": "S2"}]}, "resolvedFlowVersion": "38.00.000", "flowProperties": [], "typeOfFlow": "Other flow", "classification": {"classHierarchy": "Quantities / Environmental quantities / EPD EN 15804 / LCI indicators", "name": "GaBiCategories"}}, {"dataSetInternalID": 13, "referenceToFlowDataSet": {"shortDescription": [{"value": "Entsorgter radioaktiver Abfall (RWD)", "lang": "de"}, {"value": "Radioactive waste disposed (RWD)", "lang": "en"}], "type": "flow data set", "refObjectId": "3449546e-52ad-4b39-b809-9fb77cea8ff6", "uri": "../flows/3449546e-52ad-4b39-b809-9fb77cea8ff6.xml"}, "exchange direction": "OUTPUT", "other": {"anies": [{"name": "referenceToUnitGroupDataSet", "value": {"shortDescription": [{"value": "kg", "lang": "de"}], "type": "unit group data set", "refObjectId": "ad38d542-3fe9-439d-9b95-2f5f7752acaf", "uri": "../unitgroups/ad38d542-3fe9-439d-9b95-2f5f7752acaf.xml"}}, {"value": "0.002254", "module": "A1-A3"}, {"value": "3.097E-06", "module": "A5"}, {"value": "0.01671", "module": "B2"}, {"value": "0.001688", "module": "B5"}, {"value": "0", "module": "C1"}, {"value": "1.768E-06", "module": "C2"}, {"value": "0.0001368", "module": "C3", "scenario": "S1"}, {"value": "0", "module": "C3", "scenario": "S2"}, {"value": "0", "module": "C4"}, {"value": "-0.005843", "module": "D", "scenario": "S1"}, {"value": "0", "module": "D", "scenario": "S2"}]}, "resolvedFlowVersion": "38.00.000", "flowProperties": [], "typeOfFlow": "Other flow", "classification": {"classHierarchy": "Quantities / Environmental quantities / EPD EN 15804 / LCI indicators", "name": "GaBiCategories"}}, {"dataSetInternalID": 14, "referenceToFlowDataSet": {"shortDescription": [{"value": "Komponenten für die Wiederverwendung (CRU)", "lang": "de"}, {"value": "Components for re-use (CRU)", "lang": "en"}], "type": "flow data set", "refObjectId": "a2b32f97-3fc7-4af2-b209-525bc6426f33", "uri": "../flows/a2b32f97-3fc7-4af2-b209-525bc6426f33.xml"}, "exchange direction": "OUTPUT", "other": {"anies": [{"name": "referenceToUnitGroupDataSet", "value": {"shortDescription": [{"value": "kg", "lang": "de"}], "type": "unit group data set", "refObjectId": "ad38d542-3fe9-439d-9b95-2f5f7752acaf", "uri": "../unitgroups/ad38d542-3fe9-439d-9b95-2f5f7752acaf.xml"}}, {"value": "0", "module": "A1-A3"}, {"value": "0", "module": "A5"}, {"value": "0", "module": "B2"}, {"value": "0", "module": "B5"}, {"value": "0", "module": "C1"}, {"value": "0", "module": "C2"}, {"value": "0", "module": "C3", "scenario": "S1"}, {"value": "0", "module": "C3", "scenario": "S2"}, {"value": "0", "module": "C4"}, {"value": "0", "module": "D", "scenario": "S1"}, {"value": "0", "module": "D", "scenario": "S2"}]}, "resolvedFlowVersion": "38.00.000", "flowProperties": [], "typeOfFlow": "Other flow", "classification": {"classHierarchy": "Quantities / Environmental quantities / EPD EN 15804 / LCI indicators", "name": "GaBiCategories"}}, {"dataSetInternalID": 15, "referenceToFlowDataSet": {"shortDescription": [{"value": "Stoffe zum Recycling (MFR)", "lang": "de"}, {"value": "Materials for recycling (MFR)", "lang": "en"}], "type": "flow data set", "refObjectId": "d7fe48a5-4103-49c8-9aae-b0b5dfdbd6ae", "uri": "../flows/d7fe48a5-4103-49c8-9aae-b0b5dfdbd6ae.xml"}, "exchange direction": "OUTPUT", "other": {"anies": [{"name": "referenceToUnitGroupDataSet", "value": {"shortDescription": [{"value": "kg", "lang": "de"}], "type": "unit group data set", "refObjectId": "ad38d542-3fe9-439d-9b95-2f5f7752acaf", "uri": "../unitgroups/ad38d542-3fe9-439d-9b95-2f5f7752acaf.xml"}}, {"value": "0", "module": "A1-A3"}, {"value": "0.1169", "module": "A5"}, {"value": "0", "module": "B2"}, {"value": "0", "module": "B5"}, {"value": "0", "module": "C1"}, {"value": "0", "module": "C2"}, {"value": "0", "module": "C3", "scenario": "S1"}, {"value": "0", "module": "C3", "scenario": "S2"}, {"value": "0", "module": "C4"}, {"value": "0", "module": "D", "scenario": "S1"}, {"value": "0", "module": "D", "scenario": "S2"}]}, "resolvedFlowVersion": "38.00.000", "flowProperties": [], "typeOfFlow": "Other flow", "classification": {"classHierarchy": "Quantities / Environmental quantities / EPD EN 15804 / LCI indicators", "name": "GaBiCategories"}}, {"dataSetInternalID": 16, "referenceToFlowDataSet": {"shortDescription": [{"value": "Stoffe für die Energierückgewinnung (MER)", "lang": "de"}, {"value": "Materials for energy recovery (MER)", "lang": "en"}], "type": "flow data set", "refObjectId": "59a9181c-3aaf-46ee-8b13-2b3723b6e447", "uri": "../flows/59a9181c-3aaf-46ee-8b13-2b3723b6e447.xml"}, "exchange direction": "OUTPUT", "other": {"anies": [{"name": "referenceToUnitGroupDataSet", "value": {"shortDescription": [{"value": "kg", "lang": "de"}], "type": "unit group data set", "refObjectId": "ad38d542-3fe9-439d-9b95-2f5f7752acaf", "uri": "../unitgroups/ad38d542-3fe9-439d-9b95-2f5f7752acaf.xml"}}, {"value": "0.1741", "module": "A1-A3"}, {"value": "0.139", "module": "A5"}, {"value": "0.1232", "module": "B2"}, {"value": "0.9679", "module": "B5"}, {"value": "0", "module": "C1"}, {"value": "0", "module": "C2"}, {"value": "6.267", "module": "C3", "scenario": "S1"}, {"value": "0", "module": "C3", "scenario": "S2"}, {"value": "0", "module": "C4"}, {"value": "0", "module": "D", "scenario": "S1"}, {"value": "0", "module": "D", "scenario": "S2"}]}, "resolvedFlowVersion": "38.00.000", "flowProperties": [], "typeOfFlow": "Other flow", "classification": {"classHierarchy": "Quantities / Environmental quantities / EPD EN 15804 / LCI indicators", "name": "GaBiCategories"}}, {"dataSetInternalID": 17, "referenceToFlowDataSet": {"shortDescription": [{"value": "Exportierte elektrische Energie (EEE)", "lang": "de"}, {"value": "Exported electrical energy (EEE)", "lang": "en"}], "type": "flow data set", "refObjectId": "4da0c987-2b76-40d6-9e9e-82a017aaaf29", "uri": "../flows/4da0c987-2b76-40d6-9e9e-82a017aaaf29.xml"}, "exchange direction": "OUTPUT", "other": {"anies": [{"name": "referenceToUnitGroupDataSet", "value": {"shortDescription": [{"value": "MJ", "lang": "de"}], "type": "unit group data set", "refObjectId": "93a60a57-a3c8-11da-a746-0800200c9a66", "uri": "../unitgroups/93a60a57-a3c8-11da-a746-0800200c9a66.xml"}}, {"value": "0", "module": "A1-A3"}, {"value": "0.8232", "module": "A5"}, {"value": "0", "module": "B2"}, {"value": "2.706", "module": "B5"}, {"value": "0", "module": "C1"}, {"value": "0", "module": "C2"}, {"value": "16.4", "module": "C3", "scenario": "S1"}, {"value": "0", "module": "C3", "scenario": "S2"}, {"value": "0", "module": "C4"}, {"value": "0", "module": "D", "scenario": "S1"}, {"value": "0", "module": "D", "scenario": "S2"}]}, "resolvedFlowVersion": "38.00.000", "flowProperties": [], "typeOfFlow": "Other flow", "classification": {"classHierarchy": "Quantities / Environmental quantities / EPD EN 15804 / LCI indicators", "name": "GaBiCategories"}}, {"dataSetInternalID": 18, "referenceToFlowDataSet": {"shortDescription": [{"value": "Exportierte thermische Energie (EET)", "lang": "de"}, {"value": "Exported thermal energy (EET)", "lang": "en"}], "type": "flow data set", "refObjectId": "98daf38a-7a79-46d3-9a37-2b7bd0955810", "uri": "../flows/98daf38a-7a79-46d3-9a37-2b7bd0955810.xml"}, "exchange direction": "OUTPUT", "other": {"anies": [{"name": "referenceToUnitGroupDataSet", "value": {"shortDescription": [{"value": "MJ", "lang": "de"}], "type": "unit group data set", "refObjectId": "93a60a57-a3c8-11da-a746-0800200c9a66", "uri": "../unitgroups/93a60a57-a3c8-11da-a746-0800200c9a66.xml"}}, {"value": "0.6602", "module": "A1-A3"}, {"value": "1.465", "module": "A5"}, {"value": "0", "module": "B2"}, {"value": "4.873", "module": "B5"}, {"value": "0", "module": "C1"}, {"value": "0", "module": "C2"}, {"value": "29.45", "module": "C3", "scenario": "S1"}, {"value": "0", "module": "C3", "scenario": "S2"}, {"value": "0", "module": "C4"}, {"value": "0", "module": "D", "scenario": "S1"}, {"value": "0", "module": "D", "scenario": "S2"}]}, "resolvedFlowVersion": "38.00.000", "flowProperties": [], "typeOfFlow": "Other flow", "classification": {"classHierarchy": "Quantities / Environmental quantities / EPD EN 15804 / LCI indicators", "name": "GaBiCategories"}}]}, "LCIAResults": {"LCIAResult": [{"referenceToLCIAMethodDataSet": {"shortDescription": [{"value": "Globales Erwärmungspotenzial total (GWP-total)", "lang": "de"}, {"value": "Global Warming Potential total (GWP-total)", "lang": "en"}], "type": "LCIA method data set", "refObjectId": "6a37f984-a4b3-458a-a20a-64418c145fa2", "uri": "../lciamethods/6a37f984-a4b3-458a-a20a-64418c145fa2.xml"}, "other": {"anies": [{"name": "referenceToUnitGroupDataSet", "value": {"shortDescription": [{"value": "kg CO_(2)-Äq.", "lang": "de"}], "type": "unit group data set", "refObjectId": "1ebf3012-d0db-4de2-aefd-ef30cedb0be1", "uri": "../unitgroups/1ebf3012-d0db-4de2-aefd-ef30cedb0be1.xml"}}, {"value": "-6.803", "module": "A1-A3"}, {"value": "0.9376", "module": "A5"}, {"value": "7.037", "module": "B2"}, {"value": "1.462", "module": "B5"}, {"value": "0", "module": "C1"}, {"value": "0.07343", "module": "C2"}, {"value": "11.51", "module": "C3", "scenario": "S1"}, {"value": "11.39", "module": "C3", "scenario": "S2"}, {"value": "0", "module": "C4"}, {"value": "-4.612", "module": "D", "scenario": "S1"}, {"value": "-0.197", "module": "D", "scenario": "S2"}]}}, {"referenceToLCIAMethodDataSet": {"shortDescription": [{"value": "Globales Erwärmungspotenzial fossil (GWP-fossil)", "lang": "de"}, {"value": "Global Warming Potential fossil fuels (GWP-fossil)", "lang": "en"}], "type": "LCIA method data set", "refObjectId": "5f635281-343e-44fb-83df-1971b155e6b6", "uri": "../lciamethods/5f635281-343e-44fb-83df-1971b155e6b6.xml"}, "other": {"anies": [{"name": "referenceToUnitGroupDataSet", "value": {"shortDescription": [{"value": "kg CO_(2)-Äq.", "lang": "de"}], "type": "unit group data set", "refObjectId": "1ebf3012-d0db-4de2-aefd-ef30cedb0be1", "uri": "../unitgroups/1ebf3012-d0db-4de2-aefd-ef30cedb0be1.xml"}}, {"value": "5.313", "module": "A1-A3"}, {"value": "0.3578", "module": "A5"}, {"value": "7.028", "module": "B2"}, {"value": "1.237", "module": "B5"}, {"value": "0", "module": "C1"}, {"value": "0.07283", "module": "C2"}, {"value": "0.1675", "module": "C3", "scenario": "S1"}, {"value": "0.05482", "module": "C3", "scenario": "S2"}, {"value": "0", "module": "C4"}, {"value": "-4.609", "module": "D", "scenario": "S1"}, {"value": "-0.1959", "module": "D", "scenario": "S2"}]}}, {"referenceToLCIAMethodDataSet": {"shortDescription": [{"value": "Globales Erwärmungspotenzial biogen (GWP-biogenic)", "lang": "de"}, {"value": "Global Warming Potential biogenic (GWP-biogenic)", "lang": "en"}], "type": "LCIA method data set", "refObjectId": "2356e1ab-0185-4db5-86e5-16de51c7485c", "uri": "../lciamethods/2356e1ab-0185-4db5-86e5-16de51c7485c.xml"}, "other": {"anies": [{"name": "referenceToUnitGroupDataSet", "value": {"shortDescription": [{"value": "kg CO_(2)-Äq.", "lang": "de"}], "type": "unit group data set", "refObjectId": "1ebf3012-d0db-4de2-aefd-ef30cedb0be1", "uri": "../unitgroups/1ebf3012-d0db-4de2-aefd-ef30cedb0be1.xml"}}, {"value": "-12.14", "module": "A1-A3"}, {"value": "0.5798", "module": "A5"}, {"value": "0", "module": "B2"}, {"value": "0.2241", "module": "B5"}, {"value": "0", "module": "C1"}, {"value": "0", "module": "C2"}, {"value": "11.34", "module": "C3", "scenario": "S1"}, {"value": "11.34", "module": "C3", "scenario": "S2"}, {"value": "0", "module": "C4"}, {"value": "0", "module": "D", "scenario": "S1"}, {"value": "0", "module": "D", "scenario": "S2"}]}}, {"referenceToLCIAMethodDataSet": {"shortDescription": [{"value": "Globales Erwärmungspotenzial luluc (GWP-luluc)", "lang": "de"}, {"value": "Global Warming Potential luluc (GWP-luluc)", "lang": "en"}], "type": "LCIA method data set", "refObjectId": "4331bbdb-978a-490d-8707-eeb047f01a55", "uri": "../lciamethods/4331bbdb-978a-490d-8707-eeb047f01a55.xml"}, "other": {"anies": [{"name": "referenceToUnitGroupDataSet", "value": {"shortDescription": [{"value": "kg CO_(2)-Äq.", "lang": "de"}], "type": "unit group data set", "refObjectId": "1ebf3012-d0db-4de2-aefd-ef30cedb0be1", "uri": "../unitgroups/1ebf3012-d0db-4de2-aefd-ef30cedb0be1.xml"}}, {"value": "0.02271", "module": "A1-A3"}, {"value": "2.668E-05", "module": "A5"}, {"value": "0.009022", "module": "B2"}, {"value": "0.001121", "module": "B5"}, {"value": "0", "module": "C1"}, {"value": "0.0005959", "module": "C2"}, {"value": "0.0001075", "module": "C3", "scenario": "S1"}, {"value": "0.0001234", "module": "C3", "scenario": "S2"}, {"value": "0", "module": "C4"}, {"value": "-0.003198", "module": "D", "scenario": "S1"}, {"value": "-0.00109", "module": "D", "scenario": "S2"}]}}, {"referenceToLCIAMethodDataSet": {"shortDescription": [{"value": "Abbau Potential der stratosphärischen Ozonschicht (ODP)", "lang": "de"}, {"value": "Depletion potential of the stratospheric ozone layer (ODP)", "lang": "en"}], "type": "LCIA method data set", "refObjectId": "b5c629d6-def3-11e6-bf01-fe55135034f3", "uri": "../lciamethods/b5c629d6-def3-11e6-bf01-fe55135034f3.xml"}, "other": {"anies": [{"name": "referenceToUnitGroupDataSet", "value": {"shortDescription": [{"value": "kg CFC11-Äq.", "lang": "de"}], "type": "unit group data set", "refObjectId": "d9e957c9-7309-4474-bf3a-7777df6c4e5b", "uri": "../unitgroups/d9e957c9-7309-4474-bf3a-7777df6c4e5b.xml"}}, {"value": "1.096E-07", "module": "A1-A3"}, {"value": "3.326E-17", "module": "A5"}, {"value": "1.513E-13", "module": "B2"}, {"value": "1.557E-14", "module": "B5"}, {"value": "0", "module": "C1"}, {"value": "1.439E-17", "module": "C2"}, {"value": "1.487E-15", "module": "C3", "scenario": "S1"}, {"value": "4.587E-09", "module": "C3", "scenario": "S2"}, {"value": "0", "module": "C4"}, {"value": "-5.286E-14", "module": "D", "scenario": "S1"}, {"value": "-1.65E-08", "module": "D", "scenario": "S2"}]}}, {"referenceToLCIAMethodDataSet": {"shortDescription": [{"value": "Versauerungspotenzial von Boden und Wasser (AP)", "lang": "de"}, {"value": "Acidification potential of land and water (AP)", "lang": "en"}], "type": "LCIA method data set", "refObjectId": "b5c611c6-def3-11e6-bf01-fe55135034f3", "uri": "../lciamethods/b5c611c6-def3-11e6-bf01-fe55135034f3.xml"}, "other": {"anies": [{"name": "referenceToUnitGroupDataSet", "value": {"shortDescription": [{"value": "mol H^(+)-Äq.", "lang": "de"}], "type": "unit group data set", "refObjectId": "42e089ac-92bf-4bf2-8ca1-5fc40d18f2ed", "uri": "../unitgroups/42e089ac-92bf-4bf2-8ca1-5fc40d18f2ed.xml"}}, {"value": "0.02824", "module": "A1-A3"}, {"value": "4.545E-05", "module": "A5"}, {"value": "0.01425", "module": "B2"}, {"value": "0.002554", "module": "B5"}, {"value": "0", "module": "C1"}, {"value": "8.486E-05", "module": "C2"}, {"value": "0.001612", "module": "C3", "scenario": "S1"}, {"value": "0.0003028", "module": "C3", "scenario": "S2"}, {"value": "0", "module": "C4"}, {"value": "-0.006036", "module": "D", "scenario": "S1"}, {"value": "-0.001093", "module": "D", "scenario": "S2"}]}}, {"referenceToLCIAMethodDataSet": {"shortDescription": [{"value": "Eutrophierungspotenzial Süßwasser (EP-freshwater)", "lang": "de"}, {"value": "Eutrophication potential aquatic freshwater (EP-freshwater)", "lang": "en"}], "type": "LCIA method data set", "refObjectId": "b53ec18f-7377-4ad3-86eb-cc3f4f276b2b", "uri": "../lciamethods/b53ec18f-7377-4ad3-86eb-cc3f4f276b2b.xml"}, "other": {"anies": [{"name": "referenceToUnitGroupDataSet", "value": {"shortDescription": [{"value": "kg P-Äq.", "lang": "de"}], "type": "unit group data set", "refObjectId": "0429039d-a61d-4590-ba67-aa4a20a810a1", "uri": "../unitgroups/0429039d-a61d-4590-ba67-aa4a20a810a1.xml"}}, {"value": "0.0001647", "module": "A1-A3"}, {"value": "1.324E-08", "module": "A5"}, {"value": "0.0001699", "module": "B2"}, {"value": "2.76E-06", "module": "B5"}, {"value": "0", "module": "C1"}, {"value": "2.166E-07", "module": "C2"}, {"value": "2.038E-07", "module": "C3", "scenario": "S1"}, {"value": "5.267E-05", "module": "C3", "scenario": "S2"}, {"value": "0", "module": "C4"}, {"value": "-6.048E-06", "module": "D", "scenario": "S1"}, {"value": "-8.213E-05", "module": "D", "scenario": "S2"}]}}, {"referenceToLCIAMethodDataSet": {"shortDescription": [{"value": "Eutrophierungspotenzial Salzwasser (EP-marine)", "lang": "de"}, {"value": "Eutrophication potential aquatic marine (EP-marine)", "lang": "en"}], "type": "LCIA method data set", "refObjectId": "b5c619fa-def3-11e6-bf01-fe55135034f3", "uri": "../lciamethods/b5c619fa-def3-11e6-bf01-fe55135034f3.xml"}, "other": {"anies": [{"name": "referenceToUnitGroupDataSet", "value": {"shortDescription": [{"value": "kg N-Äq.", "lang": "de"}], "type": "unit group data set", "refObjectId": "d05bb823-ecdf-4686-8c40-bf1d9257859f", "uri": "../unitgroups/d05bb823-ecdf-4686-8c40-bf1d9257859f.xml"}}, {"value": "0.01055", "module": "A1-A3"}, {"value": "1.077E-05", "module": "A5"}, {"value": "0.00398", "module": "B2"}, {"value": "0.0006512", "module": "B5"}, {"value": "0", "module": "C1"}, {"value": "2.847E-05", "module": "C2"}, {"value": "0.0005296", "module": "C3", "scenario": "S1"}, {"value": "5.237E-05", "module": "C3", "scenario": "S2"}, {"value": "0", "module": "C4"}, {"value": "-0.001714", "module": "D", "scenario": "S1"}, {"value": "-0.0002789", "module": "D", "scenario": "S2"}]}}, {"referenceToLCIAMethodDataSet": {"shortDescription": [{"value": "Eutrophierungspotenzial Land (EP-terrestrial)", "lang": "de"}, {"value": "Eutrophication potential terrestrial (EP-terrestrial)", "lang": "en"}], "type": "LCIA method data set", "refObjectId": "b5c614d2-def3-11e6-bf01-fe55135034f3", "uri": "../lciamethods/b5c614d2-def3-11e6-bf01-fe55135034f3.xml"}, "other": {"anies": [{"name": "referenceToUnitGroupDataSet", "value": {"shortDescription": [{"value": "mol N-Äq.", "lang": "de"}], "type": "unit group data set", "refObjectId": "71b4d617-0ec9-4d3f-b65e-e438940c2401", "uri": "../unitgroups/71b4d617-0ec9-4d3f-b65e-e438940c2401.xml"}}, {"value": "0.1195", "module": "A1-A3"}, {"value": "0.0002111", "module": "A5"}, {"value": "0.03599", "module": "B2"}, {"value": "0.007253", "module": "B5"}, {"value": "0", "module": "C1"}, {"value": "0.0003359", "module": "C2"}, {"value": "0.007686", "module": "C3", "scenario": "S1"}, {"value": "0.0004964", "module": "C3", "scenario": "S2"}, {"value": "0", "module": "C4"}, {"value": "-0.01836", "module": "D", "scenario": "S1"}, {"value": "-0.002908", "module": "D", "scenario": "S2"}]}}, {"referenceToLCIAMethodDataSet": {"shortDescription": [{"value": "Bildungspotential für troposphärisches Ozon (POCP)", "lang": "de"}, {"value": "Formation potential of tropospheric ozone photochemical oxidants (POCP)", "lang": "en"}], "type": "LCIA method data set", "refObjectId": "b5c610fe-def3-11e6-bf01-fe55135034f3", "uri": "../lciamethods/b5c610fe-def3-11e6-bf01-fe55135034f3.xml"}, "other": {"anies": [{"name": "referenceToUnitGroupDataSet", "value": {"shortDescription": [{"value": "kg NMVOC-Äq.", "lang": "de"}], "type": "unit group data set", "refObjectId": "d27c25f8-fbc1-44c6-b47b-4adbae4199c6", "uri": "../unitgroups/d27c25f8-fbc1-44c6-b47b-4adbae4199c6.xml"}}, {"value": "0.04142", "module": "A1-A3"}, {"value": "3.108E-05", "module": "A5"}, {"value": "0.009879", "module": "B2"}, {"value": "0.002026", "module": "B5"}, {"value": "0", "module": "C1"}, {"value": "7.465E-05", "module": "C2"}, {"value": "0.001439", "module": "C3", "scenario": "S1"}, {"value": "0.0001295", "module": "C3", "scenario": "S2"}, {"value": "0", "module": "C4"}, {"value": "-0.004812", "module": "D", "scenario": "S1"}, {"value": "-0.0009163", "module": "D", "scenario": "S2"}]}}, {"referenceToLCIAMethodDataSet": {"shortDescription": [{"value": "Potenzial für den abiotischen Abbau nicht fossiler Ressourcen (ADPE)", "lang": "de"}, {"value": "Abiotic depletion potential for non fossil resources (ADPE)", "lang": "en"}], "type": "LCIA method data set", "refObjectId": "b2ad6494-c78d-11e6-9d9d-cec0c932ce01", "uri": "../lciamethods/b2ad6494-c78d-11e6-9d9d-cec0c932ce01.xml"}, "other": {"anies": [{"name": "referenceToUnitGroupDataSet", "value": {"shortDescription": [{"value": "kg Sb-Äq.", "lang": "de"}], "type": "unit group data set", "refObjectId": "54ccd2d9-a32a-4fc2-923d-f2c8c93e89d4", "uri": "../unitgroups/54ccd2d9-a32a-4fc2-923d-f2c8c93e89d4.xml"}}, {"value": "1.677E-05", "module": "A1-A3"}, {"value": "7.584E-10", "module": "A5"}, {"value": "1.9E-06", "module": "B2"}, {"value": "2.347E-07", "module": "B5"}, {"value": "0", "module": "C1"}, {"value": "6.462E-09", "module": "C2"}, {"value": "2.266E-08", "module": "C3", "scenario": "S1"}, {"value": "2.113E-07", "module": "C3", "scenario": "S2"}, {"value": "0", "module": "C4"}, {"value": "-7.686E-07", "module": "D", "scenario": "S1"}, {"value": "-1.942E-06", "module": "D", "scenario": "S2"}]}}, {"referenceToLCIAMethodDataSet": {"shortDescription": [{"value": "Potenzial für den abiotischen Abbau fossiler Brennstoffe (ADPF)", "lang": "de"}, {"value": "Abiotic depletion potential for fossil resources (ADPF)", "lang": "en"}], "type": "LCIA method data set", "refObjectId": "b2ad6110-c78d-11e6-9d9d-cec0c932ce01", "uri": "../lciamethods/b2ad6110-c78d-11e6-9d9d-cec0c932ce01.xml"}, "other": {"anies": [{"name": "referenceToUnitGroupDataSet", "value": {"shortDescription": [{"value": "MJ", "lang": "de"}], "type": "unit group data set", "refObjectId": "93a60a57-a3c8-11da-a746-0800200c9a66", "uri": "../unitgroups/93a60a57-a3c8-11da-a746-0800200c9a66.xml"}}, {"value": "91.4", "module": "A1-A3"}, {"value": "0.09313", "module": "A5"}, {"value": "127.8", "module": "B2"}, {"value": "26.4", "module": "B5"}, {"value": "0", "module": "C1"}, {"value": "0.971", "module": "C2"}, {"value": "2.466", "module": "C3", "scenario": "S1"}, {"value": "1.264", "module": "C3", "scenario": "S2"}, {"value": "0", "module": "C4"}, {"value": "-80", "module": "D", "scenario": "S1"}, {"value": "-3.014", "module": "D", "scenario": "S2"}]}}, {"referenceToLCIAMethodDataSet": {"shortDescription": [{"value": "Wassernutzung (WDP)", "lang": "de"}, {"value": "Water use (WDP)", "lang": "en"}], "type": "LCIA method data set", "refObjectId": "b2ad66ce-c78d-11e6-9d9d-cec0c932ce01", "uri": "../lciamethods/b2ad66ce-c78d-11e6-9d9d-cec0c932ce01.xml"}, "other": {"anies": [{"name": "referenceToUnitGroupDataSet", "value": {"shortDescription": [{"value": "m^(3) Welt-Äq. entzogen", "lang": "de"}], "type": "unit group data set", "refObjectId": "6ae2df01-888e-46c8-b17d-49fa3869b476", "uri": "../unitgroups/6ae2df01-888e-46c8-b17d-49fa3869b476.xml"}}, {"value": "1.81", "module": "A1-A3"}, {"value": "0.0375", "module": "A5"}, {"value": "1.129", "module": "B2"}, {"value": "0.4102", "module": "B5"}, {"value": "0", "module": "C1"}, {"value": "0.0006765", "module": "C2"}, {"value": "1.173", "module": "C3", "scenario": "S1"}, {"value": "0.03984", "module": "C3", "scenario": "S2"}, {"value": "0", "module": "C4"}, {"value": "-0.3547", "module": "D", "scenario": "S1"}, {"value": "-0.05001", "module": "D", "scenario": "S2"}]}}, {"referenceToLCIAMethodDataSet": {"shortDescription": [{"value": "Auftreten von Krankheiten aufgrund von Feinstaubemissionen (PM)", "lang": "de"}, {"value": "Incidence of disease due to PM emissions (PM)", "lang": "en"}], "type": "LCIA method data set", "refObjectId": "b5c602c6-def3-11e6-bf01-fe55135034f3", "uri": "../lciamethods/b5c602c6-def3-11e6-bf01-fe55135034f3.xml"}, "other": {"anies": [{"name": "referenceToUnitGroupDataSet", "value": {"shortDescription": [{"value": "Krankheitsfälle", "lang": "de"}], "type": "unit group data set", "refObjectId": "3883559b-648f-4afc-8ba2-0bd24f3affa3", "uri": "../unitgroups/3883559b-648f-4afc-8ba2-0bd24f3affa3.xml"}}, {"module": "A1-A3"}, {"module": "A5"}, {"module": "B2"}, {"module": "B5"}, {"module": "C1"}, {"module": "C2"}, {"module": "C3", "scenario": "S1"}, {"module": "C3", "scenario": "S2"}, {"module": "C4"}, {"module": "D", "scenario": "S1"}, {"module": "D", "scenario": "S2"}]}}, {"referenceToLCIAMethodDataSet": {"shortDescription": [{"value": "Wirkung durch Exposition des Menschen mit U235 (IR)", "lang": "de"}, {"value": "Human exposure efficiency relative to U235 (IR)", "lang": "en"}], "type": "LCIA method data set", "refObjectId": "b5c632be-def3-11e6-bf01-fe55135034f3", "uri": "../lciamethods/b5c632be-def3-11e6-bf01-fe55135034f3.xml"}, "other": {"anies": [{"name": "referenceToUnitGroupDataSet", "value": {"shortDescription": [{"value": "kBq U235-Äq.", "lang": "de"}], "type": "unit group data set", "refObjectId": "456b05bf-1415-44a9-9993-02452f554c09", "uri": "../unitgroups/456b05bf-1415-44a9-9993-02452f554c09.xml"}}, {"module": "A1-A3"}, {"module": "A5"}, {"module": "B2"}, {"module": "B5"}, {"module": "C1"}, {"module": "C2"}, {"module": "C3", "scenario": "S1"}, {"module": "C3", "scenario": "S2"}, {"module": "C4"}, {"module": "D", "scenario": "S1"}, {"module": "D", "scenario": "S2"}]}}, {"referenceToLCIAMethodDataSet": {"shortDescription": [{"value": "Toxizitätsvergleichseinheit für Ökosysteme (ETP-fw)", "lang": "de"}, {"value": "Comparative toxic unit for ecosystems (ETP-fw)", "lang": "en"}], "type": "LCIA method data set", "refObjectId": "ee1082d1-b0f7-43ca-a1f0-21e2a4a74511", "uri": "../lciamethods/ee1082d1-b0f7-43ca-a1f0-21e2a4a74511.xml"}, "other": {"anies": [{"name": "referenceToUnitGroupDataSet", "value": {"shortDescription": [{"value": "CTUe", "lang": "de"}], "type": "unit group data set", "refObjectId": "aa959ded-f1eb-4efb-9c5c-2d60be36b3e6", "uri": "../unitgroups/aa959ded-f1eb-4efb-9c5c-2d60be36b3e6.xml"}}, {"module": "A1-A3"}, {"module": "A5"}, {"module": "B2"}, {"module": "B5"}, {"module": "C1"}, {"module": "C2"}, {"module": "C3", "scenario": "S1"}, {"module": "C3", "scenario": "S2"}, {"module": "C4"}, {"module": "D", "scenario": "S1"}, {"module": "D", "scenario": "S2"}]}}, {"referenceToLCIAMethodDataSet": {"shortDescription": [{"value": "Toxizitätsvergleichseinheit für Menschen (krebserregend) (HTP-c)", "lang": "de"}, {"value": "Comparative toxic unit for humans (carcinogenic) (HTP-c)", "lang": "en"}], "type": "LCIA method data set", "refObjectId": "2299222a-bbd8-474f-9d4f-4dd1f18aea7c", "uri": "../lciamethods/2299222a-bbd8-474f-9d4f-4dd1f18aea7c.xml"}, "other": {"anies": [{"name": "referenceToUnitGroupDataSet", "value": {"shortDescription": [{"value": "CTUh", "lang": "de"}], "type": "unit group data set", "refObjectId": "d4c9523e-2d7e-49fd-8469-998f547d3a70", "uri": "../unitgroups/d4c9523e-2d7e-49fd-8469-998f547d3a70.xml"}}, {"module": "A1-A3"}, {"module": "A5"}, {"module": "B2"}, {"module": "B5"}, {"module": "C1"}, {"module": "C2"}, {"module": "C3", "scenario": "S1"}, {"module": "C3", "scenario": "S2"}, {"module": "C4"}, {"module": "D", "scenario": "S1"}, {"module": "D", "scenario": "S2"}]}}, {"referenceToLCIAMethodDataSet": {"shortDescription": [{"value": "Toxizitätsvergleichseinheit für Menschen (nicht krebserregend) (HTP-nc)", "lang": "de"}, {"value": "Comparative toxic unit for humans (noncarcinogenic) (HTP-nc)", "lang": "en"}], "type": "LCIA method data set", "refObjectId": "3af763a5-b7a1-48c9-9cee-1f223481fcef", "uri": "../lciamethods/3af763a5-b7a1-48c9-9cee-1f223481fcef.xml"}, "other": {"anies": [{"name": "referenceToUnitGroupDataSet", "value": {"shortDescription": [{"value": "CTUh", "lang": "de"}], "type": "unit group data set", "refObjectId": "d4c9523e-2d7e-49fd-8469-998f547d3a70", "uri": "../unitgroups/d4c9523e-2d7e-49fd-8469-998f547d3a70.xml"}}, {"module": "A1-A3"}, {"module": "A5"}, {"module": "B2"}, {"module": "B5"}, {"module": "C1"}, {"module": "C2"}, {"module": "C3", "scenario": "S1"}, {"module": "C3", "scenario": "S2"}, {"module": "C4"}, {"module": "D", "scenario": "S1"}, {"module": "D", "scenario": "S2"}]}}, {"referenceToLCIAMethodDataSet": {"shortDescription": [{"value": "Bodenqualitätsindex (SQP)", "lang": "de"}, {"value": "Soil quality index (SQP)", "lang": "en"}], "type": "LCIA method data set", "refObjectId": "b2ad6890-c78d-11e6-9d9d-cec0c932ce01", "uri": "../lciamethods/b2ad6890-c78d-11e6-9d9d-cec0c932ce01.xml"}, "other": {"anies": [{"name": "referenceToUnitGroupDataSet", "value": {"shortDescription": [{"value": "SQP", "lang": "de"}], "type": "unit group data set", "refObjectId": "f130951c-e67f-4f7f-8dd4-665de3974e18", "uri": "../unitgroups/f130951c-e67f-4f7f-8dd4-665de3974e18.xml"}}, {"module": "A1-A3"}, {"module": "A5"}, {"module": "B2"}, {"module": "B5"}, {"module": "C1"}, {"module": "C2"}, {"module": "C3", "scenario": "S1"}, {"module": "C3", "scenario": "S2"}, {"module": "C4"}, {"module": "D", "scenario": "S1"}, {"module": "D", "scenario": "S2"}]}}]}, "otherAttributes": {"{http://www.indata.network/EPD/2019}epd-version": "1.2"}, "version": "1.1", "locations": "../ILCDLocations.xml"}