{"processInformation": {"dataSetInformation": {"UUID": "55655099-d117-4e13-b173-c173122c928f", "name": {"baseName": [{"value": "TaskWorx® Carpet Tile with EcoSolution Q®, Solution Q®, or Solution Q Extreme® Face Fibre", "lang": "en"}, {"value": "TaskWorx® Carpet Tile with EcoSolution Q®, Solution Q®, or Solution Q Extreme® Face Fibre", "lang": "de"}], "functionalUnitFlowProperties": [{"lang": "en"}]}, "classificationInformation": {"classification": [{"class": [{"value": "Kunststoffe", "level": 0, "classId": "6"}, {"value": "Bodenbeläge", "level": 1, "classId": "6.2"}, {"value": "Mehrschichtig modulare Bodenbeläge", "level": 2, "classId": "6.2.06"}], "name": "OEKOBAU.DAT"}, {"class": [{"value": "02 Building products", "level": 0}, {"value": "Floor coverings", "level": 1}, {"value": "Floor coverings", "level": 2}], "name": "IBUCategories"}]}, "generalComment": [{"value": "This EPD applies to carpet tile with TaskWorx® backing system together with EcoSolution Q®, Solution Q®, or Solution Q Extreme® Nylon face fibre.\n\nTaskWorx® is a commercial carpet tile, for use as a floor covering in accordance with the manufacturers guidelines. \n\nThe carpet tile consists of Shaws unique face fibre, Nylon 6, manufactured with 1% recycled material on the TaskWorx® backing system, a modified bitumen compound with 100% natural recycled mineral filler, and a fibreglass reinforcement layer.\n\nThe EcoSolution Q®, Solution Q®, or Solution Q Extreme® face fibre is tufted into a primary backing sheet containing recycled content. Latex is added to anchor the fibre and the TaskWorx® backing system is then applied.\n\nTaskWorx® is suitable for use in all commercial settings. It has a life span of 15 years, and it comes with a 15-year warranty (subject only to installation and maintenance being carried out in line with manufacturers guidelines). \n\nThe product meets both internal and external performance standards including those established in the EU under EN 1307 and EN 10874 for a product suitable for heavy and general commercial installations.", "lang": "en"}, {"value": "Diese EPD gilt für Teppichfliesen mit TaskWorx®-Rückensystem und EcoSolution Q®-, Solution Q®- oder Solution Q Extreme®-Nylon-Deckschicht. TaskWorx® ist eine kommerzielle Teppichfliese zur Verwendung als Bodenbelag in Übereinstimmung mit den Richtlinien des Herstellers.  \n\nDie Teppichfliese besteht aus Shaws einzigartiger Oberfaser Nylon 6, die mit 1 % recyceltem Material auf dem TaskWorx®-Rückensystem hergestellt wird, einer modifizierten Bitumenmischung mit 100 % natürlichem, recyceltem Mineralfüllstoff und einer Glasfaserverstärkungsschicht. Die EcoSolution Q®, Solution Q® oder Solution Q Extreme® Oberfaser wird in eine primäre Trägerschicht getuftet, die recycelte Bestandteile enthält. Zur Verankerung der Fasern wird Latex hinzugefügt, und dann wird das TaskWorx®-Trägersystem aufgebracht. TaskWorx® ist für den Einsatz in allen gewerblichen Bereichen geeignet. Es hat eine Lebensdauer von 15 Jahren und wird mit einer 15-Jahres-Garantie geliefert (unter der Voraussetzung, dass Verlegung und Pflege gemäß den Richtlinien des Herstellers durchgeführt werden). \n\nDas Produkt erfüllt sowohl interne als auch externe Leistungsstandards, einschließlich der in der EU unter EN 1307 und EN 10874 festgelegten Standards für ein Produkt, das für schwere und allgemeine gewerbliche Installationen geeignet ist.  ", "lang": "de"}]}, "quantitativeReference": {"referenceToReferenceFlow": [0]}, "time": {"referenceYear": 2023, "dataSetValidUntil": 2028, "other": {"anies": [{"name": "publicationDateOfEPD", "value": 1699228800000}]}}, "geography": {"locationOfOperationSupplyOrProduction": {"location": "RER"}}, "technology": {"technologyDescriptionAndIncludedProcesses": [{"value": "This EPD applies to carpet tile with TaskWorx® backing system together with EcoSolution Q®, Solution Q®, or Solution Q Extreme® Nylon face fibre. TaskWorx® is a commercial carpet tile, for use as a floor covering in accordance with the manufacturer's guidelines. \nTechnical data: \nThe technical specifications of the product are listed on the products specification sheet, found at www.shawcontract.com. This product meets the requirements of the harmonized European Norm (hEN): EN14041:2004A/C:2006. Declarations of performance related to fire, electrostatic, formaldehyde emissions, and slip resistance can be found on the products specification sheet. \nDeclared unit: \nThe declaration refers to the declared unit of 1 m of installed carpet tile.", "lang": "en"}, {"value": "Diese EPD gilt für Teppichfliesen mit TaskWorx®-Rückensystem und EcoSolution Q®-, Solution Q®- oder Solution Q Extreme®-Nylon-Deckschicht. TaskWorx® ist eine kommerzielle Teppichfliese zur Verwendung als Bodenbelag in Übereinstimmung mit den Richtlinien des Herstellers.   \nTechnische Daten: \nDie technischen Daten des Produkts sind auf dem Produktdatenblatt aufgeführt, das Sie unter www.shawcontract.com finden. Dieses Produkt erfüllt die Anforderungen der harmonisierten europäischen Norm (hEN): EN14041:2004A/C:2006. Leistungserklärungen in Bezug auf Feuer, Elektrostatik, Formaldehyd-Emissionen und Rutschfestigkeit finden Sie auf dem Produktdatenblatt.   \nDeklarierte Einheit: \nDie Deklaration bezieht sich auf die deklarierte Einheit von 1 m² verlegter Teppichfliese.", "lang": "de"}], "technologicalApplicability": [{"value": "TaskWorx® Carpet Tile with EcoSolution Q®, Solution Q®, or Solution Q Extreme® Face Fibre is suitable for use as a floor covering in heavy and general commercial installations.", "lang": "en"}, {"value": "TaskWorx® Carpet Tile mit EcoSolution Q®, Solution Q® oder Solution Q Extreme®Face Fibre eignet sich für die Verwendung als Bodenbelag in schweren und allgemeinen gewerblichen Installationen.", "lang": "de"}]}}, "modellingAndValidation": {"LCIMethodAndAllocation": {"typeOfDataSet": "EPD", "referenceToLCAMethodDetails": [{"shortDescription": [{"value": "Floor coverings.pdf", "lang": "en"}], "type": "source data set", "refObjectId": "30b5f45b-0cd2-4ea3-9e35-e45ee6155bc6"}], "other": {"anies": [{"name": "subType", "value": "specific dataset"}]}}, "dataSourcesTreatmentAndRepresentativeness": {"referenceToDataSource": [{"shortDescription": [{"value": "GaBi Database (all versions)", "lang": "en"}], "type": "source data set", "refObjectId": "28d74cc0-db8b-4d7e-bc44-5f6d56ce0c4a"}, {"shortDescription": [{"value": "GaBi Database Edition 2022, CUP 2022.02", "lang": "en"}], "type": "source data set", "refObjectId": "94f442cb-662e-43ea-a792-4b0a35132e93"}], "useAdviceForDataSet": [{"value": "Scope: \nA Life Cycle Assessment (LCA) was conducted based upon production data collected from Shaw Contract (Shaw Europe, Ltd.), Plant SQ manufacturing facility (Blackaddie Road, Sanquhar, DG46DB), located in Scotland, UK. Production data was collected for TaskWorx® Carpet Tile with EcoSolution Q®, Solution Q®, or Solution Q Extreme® Face Fibre, for the period of one year, from January to December 2021.\n\nThis EPD is cradle-to-gate with options in scope with additional modules A4, A5, B1 and B2. The EPD is created in accordance to the specifications of EN 15804+A2. \n\nThe functional unit has been defined as 1m2 of installed TaskWorx® Carpet Tile.\n\nThe EPD was generated with the help of Envision LCA Tool, version 1. The tool has not been manipulated in calculating impact results. The current version of the tool is maintained, saved, and stored for 10 years to be used for revision and re-traceability purposes. \nSystem boundary: \nThe type of EPD is Cradle-to-Gate with options modules C1– C4, module D, and additional modules. The additional modules are A4, A5, B1 and B2. \n\nThe modules considered in the life cycle assessment and environmental product declaration, based on the products entire life cycle, are described as follows:\n\nProduction Stage:  \n\nModule A1 - Provision of Raw Materials.\nModule A2 - Transport of Raw Materials.\nModule A3 - Manufacturing.Construction/Installation Stage:\n\nModule A4 - Transportation by truck of the product to the construction site in Europe.\nModule A5 - Installation of the carpet, treatment of cutting waste (landfill) and packaging waste (landfill, recycling, and incineration). The production of the amount of carpet that occurs as installation waste is also included along with its transport to the place of installation. Biogenic carbon that is stored in the wooden pallets and cardboard (packaging) is released as carbon dioxide emissions into the air at the end of life in module A5.Use Stage:\n\nModule B1 - Indoor emissions of volatile organic compounds (VOCs) during the first few months after installation.\nModule B2 - Carpet cleaning per year, including vacuuming (electricity consumption) and hot water cleaning (electricity and water consumption, as well as waste water treatment).\nModule B3 - Repair (module not relevant).\nModule B4 - Replacement (module not relevant).\nModule B5 - Refurbishment (module not relevant).\nModule B6 - Operational Energy Use (module not relevant).\nModule B7 - Operational Water Use (module not relevant).End of Life Stage:\nThree scenarios have been evaluated: \nScenario 1: the TaskWorx® carpet is 100% disposed of in a landfill.\nScenario 2: the TaskWorx® carpet is 100% incinerated. \nScenario 3: 40% of TaskWorx® carpets are incinerated and the remaining 60% are landfilled. This assumption is based on the carpet disposal rates in Europe mentioned in the study conducted by Deutsche Umwelthilfe in 2017 (Umwelthilfe, 2017) and the European Commission in 2013 (Commission, 2013).\n\nModule C1 - The carpet is de-constructed manually and no additional environmental impact is caused.\nModule C2 - Transport of the carpet waste to a landfill or to the municipal waste incineration plant.\nModule C3 - Impacts from thermal treatment disposal (C3/2 and C3/3).\nModule C4 - Impacts from landfill disposal (C4/1 and C4/3).Module D includes benefits from energy recovery via treatment of packaging materials and incineration of carpets at their end of life (D/1, D/2 and D/3), as well as the burdens of balancing the secondary material content in modules A1 and A3 via the net-scrap approach.", "lang": "en"}, {"value": "Gültigkeitsbereich: \nEine Ökobilanz (LCA) wurde auf der Grundlage von Produktionsdaten durchgeführt, die von Shaw Contract (Shaw Europe, Ltd.), Werk SQ (Blackaddie Road, Sanquhar, DG46DB), in Schottland, Großbritannien, gesammelt wurden. Die Produktionsdaten wurden für TaskWorx® Carpet Tile mit EcoSolution Q®, Solution Q® oder Solution Q Extreme® Face Fibre für den Zeitraum von einem Jahr, von Januar bis Dezember 2021, erhoben.    \n\nDiese EPD umfasst alle Module von der Wiege bis zur Bahre und wurde in Übereinstimmung mit den Spezifikationen der EN 15804+A2 erstellt. Die funktionelle Einheit wurde als 1 m2 TaskWorx® Carpet Tile definiert.   \nSystemgrenze: \nDer Typ der EPD ist Cradle-to-Grave.\n\nDie in der Ökobilanz und der Umweltproduktdeklaration berücksichtigten Module, die auf dem gesamten Lebenszyklus des Produkts basieren, werden wie folgt beschrieben: Produktionsphase: Modul A1 - Bereitstellung von Rohstoffen Modul A2 - Transport von Rohstoffen Modul A3 - HerstellungBau-/Installationsphase: Modul A4 - Transport zur Baustelle Modul A5 - Montage-/Installationsverluste, einschließlich VerpackungsmaterialNutzungsphase:\n\nModul B1 - Produktnutzung/Emissionen Modul B2 - Produktwartung Modul B3 - Reparatur (Modul nicht relevant) Modul B4 - Ersatz (Modul nicht relevant) Modul B5 - Aufarbeitung (Modul nicht relevant) Modul B6 - Betrieblicher Energieverbrauch (Modul nicht relevant) Modul B7 - Betrieblicher Wasserverbrauch (Modul nicht relevant) End-of-Life-Stadium: Modul C1 - Abriss/manuelle Demontage Modul C2 - Transport zur Entsorgungsstelle Modul C3 - Abfallverarbeitung (ohne Auswirkungen deklariert) Modul C4 - EntsorgungModul D umfasst Wiederverwendungs-, Rückgewinnungs- und/oder Recyclingpotenzial. Die Gutschriften außerhalb der Systemgrenze werden berücksichtigt.", "lang": "de"}], "other": {"anies": [{"name": "referenceToOriginalEPD", "value": {"shortDescription": {"value": "TaskWorx® Carpet Tile with EcoSolution Q®, Solution Q®, or Solution Q Extreme® Face Fibre.pdf", "defaultValue": "TaskWorx® Carpet Tile with EcoSolution Q®, Solution Q®, or Solution Q Extreme® Face Fibre.pdf", "lstrings": [{"lang": "en", "value": "TaskWorx® Carpet Tile with EcoSolution Q®, Solution Q®, or Solution Q Extreme® Face Fibre.pdf"}]}, "type": "source data set", "uuid": {"uuid": "4becba0a-2727-47b4-860d-dedf77a705a7"}, "refObjectId": "4becba0a-2727-47b4-860d-dedf77a705a7", "resourceURLs": ["https://oekobaudat.de/OEKOBAU.DAT/resource/sources/4becba0a-2727-47b4-860d-dedf77a705a7/TaskWorx_Carpet_Tile_with_EcoSolution_Q_Solution_Q_or_Solution_Q_Extreme_Face_Fibre_19408.pdf?version=00.02.000"]}}]}}, "validation": {"review": [{"referenceToNameOfReviewerAndInstitution": [{"shortDescription": [{"value": "Institut Bauen und Umwelt e. V.", "lang": "en"}], "type": "contact data set", "refObjectId": "d111dbec-b024-4be5-86c5-752d6eb2cf95", "uri": "../contacts/d111dbec-b024-4be5-86c5-752d6eb2cf95.xml"}], "type": "Accredited third party review"}]}, "complianceDeclarations": {"compliance": [{"referenceToComplianceSystem": {"shortDescription": [{"value": "DIN EN 15804+A2", "lang": "en"}], "type": "source data set", "refObjectId": "c0016b33-8cf7-415c-ac6e-deba0d21440d", "uri": "../sources/c0016b33-8cf7-415c-ac6e-deba0d21440d.xml"}}, {"referenceToComplianceSystem": {"shortDescription": [{"value": "ISO 14025", "lang": "en"}], "type": "source data set", "refObjectId": "4f2eb655-6e44-4874-a95a-e28f5442cd4d", "uri": "../sources/4f2eb655-6e44-4874-a95a-e28f5442cd4d.xml"}}]}}, "administrativeInformation": {"commissionerAndGoal": {"referenceToCommissioner": [{"shortDescription": [{"value": "Shaw Contract (Shaw Europe Ltd.)", "lang": "en"}], "type": "contact data set", "refObjectId": "5e5cda45-67f4-4c23-9983-a2c2835c74a0", "uri": "../contacts/5e5cda45-67f4-4c23-9983-a2c2835c74a0.xml"}]}, "dataGenerator": {"referenceToPersonOrEntityGeneratingTheDataSet": [{"shortDescription": [{"value": "Sphera Solutions GmbH", "lang": "en"}], "type": "contact data set", "refObjectId": "623edf96-39d1-4e6f-9892-674c7228546b", "uri": "../contacts/623edf96-39d1-4e6f-9892-674c7228546b.xml"}]}, "dataEntryBy": {"timeStamp": 1699228800000, "referenceToDataSetFormat": [{"shortDescription": [{"value": "ILCD Format", "lang": "en"}], "type": "source data set", "refObjectId": "a97a0155-0234-4b87-b4ce-a45da52f2a40", "uri": "../sources/a97a0155-0234-4b87-b4ce-a45da52f2a40.xml"}, {"shortDescription": [{"value": "EPD-Datenformaterweiterungen v1.2", "lang": "de"}, {"value": "EPD Data Format Extensions v1.2", "lang": "en"}], "type": "source data set", "refObjectId": "a29449fd-aa2f-4de8-b5d7-4b06b43c6fde", "uri": "../sources/a29449fd-aa2f-4de8-b5d7-4b06b43c6fde.xml"}]}, "publicationAndOwnership": {"dataSetVersion": "00.04.000", "referenceToRegistrationAuthority": {"shortDescription": [{"value": "Institut Bauen und Umwelt e. V.", "lang": "en"}], "type": "contact data set", "refObjectId": "d111dbec-b024-4be5-86c5-752d6eb2cf95", "uri": "../contacts/d111dbec-b024-4be5-86c5-752d6eb2cf95.xml"}, "registrationNumber": "EPD-SHA-20230443-CBA1-EN", "referenceToOwnershipOfDataSet": {"shortDescription": [{"value": "Shaw Contract (Shaw Europe Ltd.)", "lang": "en"}], "type": "contact data set", "refObjectId": "5e5cda45-67f4-4c23-9983-a2c2835c74a0", "uri": "../contacts/5e5cda45-67f4-4c23-9983-a2c2835c74a0.xml"}, "copyright": true, "licenseType": "Free of charge for all users and uses", "accessRestrictions": [{"value": "None", "lang": "en"}], "other": {"anies": [{"name": "referenceToPublisher", "value": {"shortDescription": [{"value": "Institut Bauen und Umwelt e. V.", "lang": "en"}], "type": "contact data set", "refObjectId": "d111dbec-b024-4be5-86c5-752d6eb2cf95", "uri": "../contacts/d111dbec-b024-4be5-86c5-752d6eb2cf95.xml"}}]}}}, "exchanges": {"exchange": [{"dataSetInternalID": 0, "referenceToFlowDataSet": {"shortDescription": [{"value": "TaskWorx® Carpet (TaskWorx® Carpet Tile with EcoSolution Q®, Solution Q®, or Solution Q Extreme® Face Fibre)", "lang": "en"}], "type": "flow data set", "refObjectId": "b3d27dac-ab87-fe10-6026-42c893aef599", "uri": "../flows/b3d27dac-ab87-fe10-6026-42c893aef599.xml"}, "meanAmount": 1.0, "referencesToDataSource": {}, "referenceFlow": true, "resolvedFlowVersion": "00.04.000", "resultingflowAmount": 1.0, "flowProperties": [{"name": [{"lang": "en", "value": "Area"}, {"lang": "de", "value": "Fläche"}], "uuid": "93a60a56-a3c8-19da-a746-0800200c9a66", "referenceFlowProperty": true, "meanValue": 1.0, "referenceUnit": "qm", "unitGroupUUID": "c20a03d7-bd90-4569-bc94-66cfd364dfc8"}], "materialProperties": [{"name": "grammage", "value": "4.292", "unit": "kg/m^2", "unitDescription": "kilograms per square meter"}, {"name": "layer thickness", "value": "0.007", "unit": "m", "unitDescription": "meters"}], "typeOfFlow": "Product flow", "classification": {"classHierarchy": "Kunststoffe / Bodenbeläge / Mehrschichtig modulare Bodenbeläge", "name": "OEKOBAU.DAT"}}, {"dataSetInternalID": 1, "referenceToFlowDataSet": {"shortDescription": [{"value": "Renewable primary energy as energy carrier (PERE)", "lang": "en"}, {"value": "Erneuerbare Primärenergie als Energieträger (PERE)", "lang": "de"}], "type": "flow data set", "refObjectId": "20f32be5-0398-4288-9b6d-accddd195317", "uri": "../flows/20f32be5-0398-4288-9b6d-accddd195317.xml"}, "exchange direction": "INPUT", "other": {"anies": [{"name": "referenceToUnitGroupDataSet", "value": {"shortDescription": [{"value": "MJ", "lang": "en"}], "type": "unit group data set", "refObjectId": "93a60a57-a3c8-11da-a746-0800200c9a66", "uri": "../unitgroups/93a60a57-a3c8-11da-a746-0800200c9a66.xml"}}, {"value": "10.5392708706242", "module": "A1-A3"}, {"value": "0.213261200934813", "module": "A4"}, {"value": "5.11179196110649", "module": "A5"}, {"value": "0", "module": "B1"}, {"value": "2.88178210974505", "module": "B2"}, {"value": "0", "module": "C1"}, {"value": "0.043999088317108", "module": "C2"}, {"value": "0", "module": "C3"}, {"value": "0.354836140956133", "module": "C4"}, {"value": "0.0280788525963481", "module": "D"}]}, "resolvedFlowVersion": "38.00.000", "flowProperties": [], "typeOfFlow": "Other flow", "classification": {"classHierarchy": "Quantities", "name": "GaBiCategories"}}, {"dataSetInternalID": 2, "referenceToFlowDataSet": {"shortDescription": [{"value": "Renewable primary energy resources as material utilization (PERM)", "lang": "en"}, {"value": "Erneuerbare Primärenergie zur stofflichen Nutzung (PERM)", "lang": "de"}], "type": "flow data set", "refObjectId": "fb3ec0de-548d-4508-aea5-00b73bf6f702", "uri": "../flows/fb3ec0de-548d-4508-aea5-00b73bf6f702.xml"}, "exchange direction": "INPUT", "other": {"anies": [{"name": "referenceToUnitGroupDataSet", "value": {"shortDescription": [{"value": "MJ", "lang": "en"}], "type": "unit group data set", "refObjectId": "93a60a57-a3c8-11da-a746-0800200c9a66", "uri": "../unitgroups/93a60a57-a3c8-11da-a746-0800200c9a66.xml"}}, {"value": "5.306440264", "module": "A1-A3"}, {"value": "0", "module": "A4"}, {"value": "-4.188556345342", "module": "A5"}, {"value": "0", "module": "B1"}, {"value": "0", "module": "B2"}, {"value": "0", "module": "C1"}, {"value": "0", "module": "C2"}, {"value": "0", "module": "C3"}, {"value": "0", "module": "C4"}, {"value": "0", "module": "D"}]}, "resolvedFlowVersion": "38.00.000", "flowProperties": [], "typeOfFlow": "Other flow", "classification": {"classHierarchy": "Quantities", "name": "GaBiCategories"}}, {"dataSetInternalID": 3, "referenceToFlowDataSet": {"shortDescription": [{"value": "Total use of renewable primary energy resources (PERT)", "lang": "en"}, {"value": "Total erneuerbare Primärenergie (PERT)", "lang": "de"}], "type": "flow data set", "refObjectId": "53f97275-fa8a-4cdd-9024-65936002acd0", "uri": "../flows/53f97275-fa8a-4cdd-9024-65936002acd0.xml"}, "exchange direction": "INPUT", "other": {"anies": [{"name": "referenceToUnitGroupDataSet", "value": {"shortDescription": [{"value": "MJ", "lang": "en"}], "type": "unit group data set", "refObjectId": "93a60a57-a3c8-11da-a746-0800200c9a66", "uri": "../unitgroups/93a60a57-a3c8-11da-a746-0800200c9a66.xml"}}, {"value": "15.8457111346242", "module": "A1-A3"}, {"value": "0.213261200934813", "module": "A4"}, {"value": "0.923235615764485", "module": "A5"}, {"value": "0", "module": "B1"}, {"value": "2.88178210974505", "module": "B2"}, {"value": "0", "module": "C1"}, {"value": "0.043999088317108", "module": "C2"}, {"value": "0", "module": "C3"}, {"value": "0.354836140956133", "module": "C4"}, {"value": "0.0280788525963481", "module": "D"}]}, "resolvedFlowVersion": "38.00.000", "flowProperties": [], "typeOfFlow": "Other flow", "classification": {"classHierarchy": "Quantities / Environmental quantities / EPD EN 15804 / LCI indicators", "name": "GaBiCategories"}}, {"dataSetInternalID": 4, "referenceToFlowDataSet": {"shortDescription": [{"value": "Non renewable primary energy as energy carrier (PENRE)", "lang": "en"}, {"value": "Nicht-erneuerbare Primärenergie als Energieträger (PENRE)", "lang": "de"}], "type": "flow data set", "refObjectId": "ac857178-2b45-46ec-892a-a9a4332f0372", "uri": "../flows/ac857178-2b45-46ec-892a-a9a4332f0372.xml"}, "exchange direction": "INPUT", "other": {"anies": [{"name": "referenceToUnitGroupDataSet", "value": {"shortDescription": [{"value": "MJ", "lang": "en"}], "type": "unit group data set", "refObjectId": "93a60a57-a3c8-11da-a746-0800200c9a66", "uri": "../unitgroups/93a60a57-a3c8-11da-a746-0800200c9a66.xml"}}, {"value": "132.461212167574", "module": "A1-A3"}, {"value": "3.76034938001455", "module": "A4"}, {"value": "1.59452277083176", "module": "A5"}, {"value": "0", "module": "B1"}, {"value": "5.19304085499709", "module": "B2"}, {"value": "0", "module": "C1"}, {"value": "0.775818309890393", "module": "C2"}, {"value": "0", "module": "C3"}, {"value": "4.31830118768704", "module": "C4"}, {"value": "0.854953958336337", "module": "D"}]}, "resolvedFlowVersion": "38.00.000", "flowProperties": [], "typeOfFlow": "Other flow", "classification": {"classHierarchy": "Quantities", "name": "GaBiCategories"}}, {"dataSetInternalID": 5, "referenceToFlowDataSet": {"shortDescription": [{"value": "Non renewable primary energy as material utilization (PENRM)", "lang": "en"}, {"value": "Nicht-erneuerbare Primärenergie zur stofflichen Nutzung (PENRM)", "lang": "de"}], "type": "flow data set", "refObjectId": "1421caa0-679d-4bf4-b282-0eb850ccae27", "uri": "../flows/1421caa0-679d-4bf4-b282-0eb850ccae27.xml"}, "exchange direction": "INPUT", "other": {"anies": [{"name": "referenceToUnitGroupDataSet", "value": {"shortDescription": [{"value": "MJ", "lang": "en"}], "type": "unit group data set", "refObjectId": "93a60a57-a3c8-11da-a746-0800200c9a66", "uri": "../unitgroups/93a60a57-a3c8-11da-a746-0800200c9a66.xml"}}, {"value": "58.483894097", "module": "A1-A3"}, {"value": "0", "module": "A4"}, {"value": "-0.316781634121", "module": "A5"}, {"value": "0", "module": "B1"}, {"value": "0", "module": "B2"}, {"value": "0", "module": "C1"}, {"value": "0", "module": "C2"}, {"value": "0", "module": "C3"}, {"value": "0", "module": "C4"}, {"value": "0", "module": "D"}]}, "resolvedFlowVersion": "38.00.000", "flowProperties": [], "typeOfFlow": "Other flow", "classification": {"classHierarchy": "Quantities", "name": "GaBiCategories"}}, {"dataSetInternalID": 6, "referenceToFlowDataSet": {"shortDescription": [{"value": "Total use of non renewable primary energy resources (PENRT)", "lang": "en"}, {"value": "Total nicht erneuerbare Primärenergie (PENRT)", "lang": "de"}], "type": "flow data set", "refObjectId": "06159210-646b-4c8d-8583-da9b3b95a6c1", "uri": "../flows/06159210-646b-4c8d-8583-da9b3b95a6c1.xml"}, "exchange direction": "INPUT", "other": {"anies": [{"name": "referenceToUnitGroupDataSet", "value": {"shortDescription": [{"value": "MJ", "lang": "en"}], "type": "unit group data set", "refObjectId": "93a60a57-a3c8-11da-a746-0800200c9a66", "uri": "../unitgroups/93a60a57-a3c8-11da-a746-0800200c9a66.xml"}}, {"value": "189.273568991685", "module": "A1-A3"}, {"value": "3.76034938001455", "module": "A4"}, {"value": "1.27774113671077", "module": "A5"}, {"value": "0", "module": "B1"}, {"value": "5.19304085499712", "module": "B2"}, {"value": "0", "module": "C1"}, {"value": "0.775818309890393", "module": "C2"}, {"value": "0", "module": "C3"}, {"value": "4.31830118768708", "module": "C4"}, {"value": "0.854953958336349", "module": "D"}]}, "resolvedFlowVersion": "38.00.000", "flowProperties": [], "typeOfFlow": "Other flow", "classification": {"classHierarchy": "Quantities / Environmental quantities / EPD EN 15804 / LCI indicators", "name": "GaBiCategories"}}, {"dataSetInternalID": 7, "referenceToFlowDataSet": {"shortDescription": [{"value": "Use of secondary material (SM)", "lang": "en"}, {"value": "Einsatz von Sekundärstoffen (SM)", "lang": "de"}], "type": "flow data set", "refObjectId": "c6a1f35f-2d09-4f54-8dfb-97e502e1ce92", "uri": "../flows/c6a1f35f-2d09-4f54-8dfb-97e502e1ce92.xml"}, "exchange direction": "INPUT", "other": {"anies": [{"name": "referenceToUnitGroupDataSet", "value": {"shortDescription": [{"value": "kg", "lang": "en"}], "type": "unit group data set", "refObjectId": "ad38d542-3fe9-439d-9b95-2f5f7752acaf", "uri": "../unitgroups/ad38d542-3fe9-439d-9b95-2f5f7752acaf.xml"}}, {"value": "2.34392823168497", "module": "A1-A3"}, {"value": "0", "module": "A4"}, {"value": "0.123364643772893", "module": "A5"}, {"value": "0", "module": "B1"}, {"value": "0", "module": "B2"}, {"value": "0", "module": "C1"}, {"value": "0", "module": "C2"}, {"value": "0", "module": "C3"}, {"value": "0", "module": "C4"}, {"value": "-2.46729287545786", "module": "D"}]}, "resolvedFlowVersion": "38.00.000", "flowProperties": [], "typeOfFlow": "Other flow", "classification": {"classHierarchy": "Quantities / Environmental quantities / EPD EN 15804 / LCI indicators", "name": "GaBiCategories"}}, {"dataSetInternalID": 8, "referenceToFlowDataSet": {"shortDescription": [{"value": "Use of renewable secondary fuels (RSF)", "lang": "en"}, {"value": "Erneuerbare Sekundärbrennstoffe (RSF)", "lang": "de"}], "type": "flow data set", "refObjectId": "64333088-a55f-4aa2-9a31-c10b07816787", "uri": "../flows/64333088-a55f-4aa2-9a31-c10b07816787.xml"}, "exchange direction": "INPUT", "other": {"anies": [{"name": "referenceToUnitGroupDataSet", "value": {"shortDescription": [{"value": "MJ", "lang": "en"}], "type": "unit group data set", "refObjectId": "93a60a57-a3c8-11da-a746-0800200c9a66", "uri": "../unitgroups/93a60a57-a3c8-11da-a746-0800200c9a66.xml"}}, {"value": "0", "module": "A1-A3"}, {"value": "0", "module": "A4"}, {"value": "0", "module": "A5"}, {"value": "0", "module": "B1"}, {"value": "0", "module": "B2"}, {"value": "0", "module": "C1"}, {"value": "0", "module": "C2"}, {"value": "0", "module": "C3"}, {"value": "0", "module": "C4"}, {"value": "0", "module": "D"}]}, "resolvedFlowVersion": "38.00.000", "flowProperties": [], "typeOfFlow": "Other flow", "classification": {"classHierarchy": "Quantities / Environmental quantities / EPD EN 15804 / LCI indicators", "name": "GaBiCategories"}}, {"dataSetInternalID": 9, "referenceToFlowDataSet": {"shortDescription": [{"value": "Use of non renewable secondary fuels (NRSF)", "lang": "en"}, {"value": "Nicht erneuerbare Sekundärbrennstoffe (NRSF)", "lang": "de"}], "type": "flow data set", "refObjectId": "89def144-d39a-4287-b86f-efde453ddcb2", "uri": "../flows/89def144-d39a-4287-b86f-efde453ddcb2.xml"}, "exchange direction": "INPUT", "other": {"anies": [{"name": "referenceToUnitGroupDataSet", "value": {"shortDescription": [{"value": "MJ", "lang": "en"}], "type": "unit group data set", "refObjectId": "93a60a57-a3c8-11da-a746-0800200c9a66", "uri": "../unitgroups/93a60a57-a3c8-11da-a746-0800200c9a66.xml"}}, {"value": "0", "module": "A1-A3"}, {"value": "0", "module": "A4"}, {"value": "0", "module": "A5"}, {"value": "0", "module": "B1"}, {"value": "0", "module": "B2"}, {"value": "0", "module": "C1"}, {"value": "0", "module": "C2"}, {"value": "0", "module": "C3"}, {"value": "0", "module": "C4"}, {"value": "0", "module": "D"}]}, "resolvedFlowVersion": "38.00.000", "flowProperties": [], "typeOfFlow": "Other flow", "classification": {"classHierarchy": "Quantities / Environmental quantities / EPD EN 15804 / LCI indicators", "name": "GaBiCategories"}}, {"dataSetInternalID": 10, "referenceToFlowDataSet": {"shortDescription": [{"value": "Use of net fresh water (FW)", "lang": "en"}, {"value": "Einsatz von Süßwasserressourcen (FW)", "lang": "de"}], "type": "flow data set", "refObjectId": "3cf952c8-f3a4-461d-8c96-96456ca62246", "uri": "../flows/3cf952c8-f3a4-461d-8c96-96456ca62246.xml"}, "exchange direction": "INPUT", "other": {"anies": [{"name": "referenceToUnitGroupDataSet", "value": {"shortDescription": [{"value": "m^3", "lang": "en"}], "type": "unit group data set", "refObjectId": "cd950537-0a98-4044-9ba7-9f9a68d0a504", "uri": "../unitgroups/cd950537-0a98-4044-9ba7-9f9a68d0a504.xml"}}, {"value": "0.0282878083654561", "module": "A1-A3"}, {"value": "0.000229128176083469", "module": "A4"}, {"value": "0.00956253596591696", "module": "A5"}, {"value": "0", "module": "B1"}, {"value": "0.00275246950798643", "module": "B2"}, {"value": "0", "module": "C1"}, {"value": "4.97607273751046E-05", "module": "C2"}, {"value": "0", "module": "C3"}, {"value": "5.58723466881523E-05", "module": "C4"}, {"value": "1.66980893623308E-05", "module": "D"}]}, "resolvedFlowVersion": "38.00.000", "flowProperties": [], "typeOfFlow": "Other flow", "classification": {"classHierarchy": "Quantities / Environmental quantities / EPD EN 15804 / LCI indicators", "name": "GaBiCategories"}}, {"dataSetInternalID": 11, "referenceToFlowDataSet": {"shortDescription": [{"value": "Hazardous waste disposed (HWD)", "lang": "en"}, {"value": "Gefährlicher Abfall zur Deponie (HWD)", "lang": "de"}], "type": "flow data set", "refObjectId": "430f9e0f-59b2-46a0-8e0d-55e0e84948fc", "uri": "../flows/430f9e0f-59b2-46a0-8e0d-55e0e84948fc.xml"}, "exchange direction": "OUTPUT", "other": {"anies": [{"name": "referenceToUnitGroupDataSet", "value": {"shortDescription": [{"value": "kg", "lang": "en"}], "type": "unit group data set", "refObjectId": "ad38d542-3fe9-439d-9b95-2f5f7752acaf", "uri": "../unitgroups/ad38d542-3fe9-439d-9b95-2f5f7752acaf.xml"}}, {"value": "8.41815527471676E-07", "module": "A1-A3"}, {"value": "1.71070388491403E-11", "module": "A4"}, {"value": "4.67466227664652E-08", "module": "A5"}, {"value": "0", "module": "B1"}, {"value": "4.49352124421946E-10", "module": "B2"}, {"value": "0", "module": "C1"}, {"value": "3.71520740451096E-12", "module": "C2"}, {"value": "0", "module": "C3"}, {"value": "6.65793054628155E-10", "module": "C4"}, {"value": "1.19358638108094E-10", "module": "D"}]}, "resolvedFlowVersion": "38.00.000", "flowProperties": [], "typeOfFlow": "Other flow", "classification": {"classHierarchy": "Quantities / Environmental quantities / EPD EN 15804 / LCI indicators", "name": "GaBiCategories"}}, {"dataSetInternalID": 12, "referenceToFlowDataSet": {"shortDescription": [{"value": "Non hazardous waste disposed (NHWD)", "lang": "en"}, {"value": "Entsorgter nicht gefährlicher Abfall (NHWD)", "lang": "de"}], "type": "flow data set", "refObjectId": "b29ef66b-e286-4afa-949f-62f1a7b4d7fa", "uri": "../flows/b29ef66b-e286-4afa-949f-62f1a7b4d7fa.xml"}, "exchange direction": "OUTPUT", "other": {"anies": [{"name": "referenceToUnitGroupDataSet", "value": {"shortDescription": [{"value": "kg", "lang": "en"}], "type": "unit group data set", "refObjectId": "ad38d542-3fe9-439d-9b95-2f5f7752acaf", "uri": "../unitgroups/ad38d542-3fe9-439d-9b95-2f5f7752acaf.xml"}}, {"value": "0.32152663645538", "module": "A1-A3"}, {"value": "0.000511966714435075", "module": "A4"}, {"value": "0.270583152305935", "module": "A5"}, {"value": "0", "module": "B1"}, {"value": "0.00477223121960601", "module": "B2"}, {"value": "0", "module": "C1"}, {"value": "0.000111185959481697", "module": "C2"}, {"value": "0", "module": "C3"}, {"value": "4.27491945346628", "module": "C4"}, {"value": "7.32876457688988E-05", "module": "D"}]}, "resolvedFlowVersion": "38.00.000", "flowProperties": [], "typeOfFlow": "Other flow", "classification": {"classHierarchy": "Quantities / Environmental quantities / EPD EN 15804 / LCI indicators", "name": "GaBiCategories"}}, {"dataSetInternalID": 13, "referenceToFlowDataSet": {"shortDescription": [{"value": "Radioactive waste disposed (RWD)", "lang": "en"}, {"value": "Entsorgter radioaktiver Abfall (RWD)", "lang": "de"}], "type": "flow data set", "refObjectId": "3449546e-52ad-4b39-b809-9fb77cea8ff6", "uri": "../flows/3449546e-52ad-4b39-b809-9fb77cea8ff6.xml"}, "exchange direction": "OUTPUT", "other": {"anies": [{"name": "referenceToUnitGroupDataSet", "value": {"shortDescription": [{"value": "kg", "lang": "en"}], "type": "unit group data set", "refObjectId": "ad38d542-3fe9-439d-9b95-2f5f7752acaf", "uri": "../unitgroups/ad38d542-3fe9-439d-9b95-2f5f7752acaf.xml"}}, {"value": "0.00412908213982618", "module": "A1-A3"}, {"value": "4.39995111015045E-06", "module": "A4"}, {"value": "0.000237295159416604", "module": "A5"}, {"value": "0", "module": "B1"}, {"value": "0.000829748839831687", "module": "B2"}, {"value": "0", "module": "C1"}, {"value": "9.55555843888123E-07", "module": "C2"}, {"value": "0", "module": "C3"}, {"value": "5.30350205626825E-05", "module": "C4"}, {"value": "5.62071320731152E-07", "module": "D"}]}, "resolvedFlowVersion": "38.00.000", "flowProperties": [], "typeOfFlow": "Other flow", "classification": {"classHierarchy": "Quantities / Environmental quantities / EPD EN 15804 / LCI indicators", "name": "GaBiCategories"}}, {"dataSetInternalID": 14, "referenceToFlowDataSet": {"shortDescription": [{"value": "Components for re-use (CRU)", "lang": "en"}, {"value": "Komponenten für die Wiederverwendung (CRU)", "lang": "de"}], "type": "flow data set", "refObjectId": "a2b32f97-3fc7-4af2-b209-525bc6426f33", "uri": "../flows/a2b32f97-3fc7-4af2-b209-525bc6426f33.xml"}, "exchange direction": "OUTPUT", "other": {"anies": [{"name": "referenceToUnitGroupDataSet", "value": {"shortDescription": [{"value": "kg", "lang": "en"}], "type": "unit group data set", "refObjectId": "ad38d542-3fe9-439d-9b95-2f5f7752acaf", "uri": "../unitgroups/ad38d542-3fe9-439d-9b95-2f5f7752acaf.xml"}}, {"value": "0", "module": "A1-A3"}, {"value": "0", "module": "A4"}, {"value": "0", "module": "A5"}, {"value": "0", "module": "B1"}, {"value": "0", "module": "B2"}, {"value": "0", "module": "C1"}, {"value": "0", "module": "C2"}, {"value": "0", "module": "C3"}, {"value": "0", "module": "C4"}, {"value": "0", "module": "D"}]}, "resolvedFlowVersion": "38.00.000", "flowProperties": [], "typeOfFlow": "Other flow", "classification": {"classHierarchy": "Quantities / Environmental quantities / EPD EN 15804 / LCI indicators", "name": "GaBiCategories"}}, {"dataSetInternalID": 15, "referenceToFlowDataSet": {"shortDescription": [{"value": "Materials for recycling (MFR)", "lang": "en"}, {"value": "Stoffe zum Recycling (MFR)", "lang": "de"}], "type": "flow data set", "refObjectId": "d7fe48a5-4103-49c8-9aae-b0b5dfdbd6ae", "uri": "../flows/d7fe48a5-4103-49c8-9aae-b0b5dfdbd6ae.xml"}, "exchange direction": "OUTPUT", "other": {"anies": [{"name": "referenceToUnitGroupDataSet", "value": {"shortDescription": [{"value": "kg", "lang": "en"}], "type": "unit group data set", "refObjectId": "ad38d542-3fe9-439d-9b95-2f5f7752acaf", "uri": "../unitgroups/ad38d542-3fe9-439d-9b95-2f5f7752acaf.xml"}}, {"value": "0", "module": "A1-A3"}, {"value": "0", "module": "A4"}, {"value": "0.1809136631583", "module": "A5"}, {"value": "0", "module": "B1"}, {"value": "0", "module": "B2"}, {"value": "0", "module": "C1"}, {"value": "0", "module": "C2"}, {"value": "0", "module": "C3"}, {"value": "0", "module": "C4"}, {"value": "0", "module": "D"}]}, "resolvedFlowVersion": "38.00.000", "flowProperties": [], "typeOfFlow": "Other flow", "classification": {"classHierarchy": "Quantities / Environmental quantities / EPD EN 15804 / LCI indicators", "name": "GaBiCategories"}}, {"dataSetInternalID": 16, "referenceToFlowDataSet": {"shortDescription": [{"value": "Materials for energy recovery (MER)", "lang": "en"}, {"value": "Stoffe für die Energierückgewinnung (MER)", "lang": "de"}], "type": "flow data set", "refObjectId": "59a9181c-3aaf-46ee-8b13-2b3723b6e447", "uri": "../flows/59a9181c-3aaf-46ee-8b13-2b3723b6e447.xml"}, "exchange direction": "OUTPUT", "other": {"anies": [{"name": "referenceToUnitGroupDataSet", "value": {"shortDescription": [{"value": "kg", "lang": "en"}], "type": "unit group data set", "refObjectId": "ad38d542-3fe9-439d-9b95-2f5f7752acaf", "uri": "../unitgroups/ad38d542-3fe9-439d-9b95-2f5f7752acaf.xml"}}, {"value": "0", "module": "A1-A3"}, {"value": "0", "module": "A4"}, {"value": "0", "module": "A5"}, {"value": "0", "module": "B1"}, {"value": "0", "module": "B2"}, {"value": "0", "module": "C1"}, {"value": "0", "module": "C2"}, {"value": "0", "module": "C3"}, {"value": "0", "module": "C4"}, {"value": "0", "module": "D"}]}, "resolvedFlowVersion": "38.00.000", "flowProperties": [], "typeOfFlow": "Other flow", "classification": {"classHierarchy": "Quantities / Environmental quantities / EPD EN 15804 / LCI indicators", "name": "GaBiCategories"}}, {"dataSetInternalID": 17, "referenceToFlowDataSet": {"shortDescription": [{"value": "Exported electrical energy (EEE)", "lang": "en"}, {"value": "Exportierte elektrische Energie (EEE)", "lang": "de"}], "type": "flow data set", "refObjectId": "4da0c987-2b76-40d6-9e9e-82a017aaaf29", "uri": "../flows/4da0c987-2b76-40d6-9e9e-82a017aaaf29.xml"}, "exchange direction": "OUTPUT", "other": {"anies": [{"name": "referenceToUnitGroupDataSet", "value": {"shortDescription": [{"value": "MJ", "lang": "en"}], "type": "unit group data set", "refObjectId": "93a60a57-a3c8-11da-a746-0800200c9a66", "uri": "../unitgroups/93a60a57-a3c8-11da-a746-0800200c9a66.xml"}}, {"value": "0", "module": "A1-A3"}, {"value": "0", "module": "A4"}, {"value": "0.0636508991090627", "module": "A5"}, {"value": "0", "module": "B1"}, {"value": "0", "module": "B2"}, {"value": "0", "module": "C1"}, {"value": "0", "module": "C2"}, {"value": "0", "module": "C3"}, {"value": "0", "module": "C4"}, {"value": "0", "module": "D"}]}, "resolvedFlowVersion": "38.00.000", "flowProperties": [], "typeOfFlow": "Other flow", "classification": {"classHierarchy": "Quantities / Environmental quantities / EPD EN 15804 / LCI indicators", "name": "GaBiCategories"}}, {"dataSetInternalID": 18, "referenceToFlowDataSet": {"shortDescription": [{"value": "Exported thermal energy (EET)", "lang": "en"}, {"value": "Exportierte thermische Energie (EET)", "lang": "de"}], "type": "flow data set", "refObjectId": "98daf38a-7a79-46d3-9a37-2b7bd0955810", "uri": "../flows/98daf38a-7a79-46d3-9a37-2b7bd0955810.xml"}, "exchange direction": "OUTPUT", "other": {"anies": [{"name": "referenceToUnitGroupDataSet", "value": {"shortDescription": [{"value": "MJ", "lang": "en"}], "type": "unit group data set", "refObjectId": "93a60a57-a3c8-11da-a746-0800200c9a66", "uri": "../unitgroups/93a60a57-a3c8-11da-a746-0800200c9a66.xml"}}, {"value": "0", "module": "A1-A3"}, {"value": "0", "module": "A4"}, {"value": "0.0976949264004296", "module": "A5"}, {"value": "0", "module": "B1"}, {"value": "0", "module": "B2"}, {"value": "0", "module": "C1"}, {"value": "0", "module": "C2"}, {"value": "0", "module": "C3"}, {"value": "0", "module": "C4"}, {"value": "0", "module": "D"}]}, "resolvedFlowVersion": "38.00.000", "flowProperties": [], "typeOfFlow": "Other flow", "classification": {"classHierarchy": "Quantities / Environmental quantities / EPD EN 15804 / LCI indicators", "name": "GaBiCategories"}}]}, "LCIAResults": {"LCIAResult": [{"referenceToLCIAMethodDataSet": {"shortDescription": [{"value": "Global Warming Potential total (GWP-total)", "lang": "en"}, {"value": "Globales Erwärmungspotenzial total (GWP-total)", "lang": "de"}], "type": "LCIA method data set", "refObjectId": "6a37f984-a4b3-458a-a20a-64418c145fa2", "uri": "../lciamethods/6a37f984-a4b3-458a-a20a-64418c145fa2.xml"}, "other": {"anies": [{"name": "referenceToUnitGroupDataSet", "value": {"shortDescription": [{"value": "kg CO_(2) eq", "lang": "en"}], "type": "unit group data set", "refObjectId": "1ebf3012-d0db-4de2-aefd-ef30cedb0be1", "uri": "../unitgroups/1ebf3012-d0db-4de2-aefd-ef30cedb0be1.xml"}}, {"value": "7.80772589443914", "module": "A1-A3"}, {"value": "0.26770905911227", "module": "A4"}, {"value": "0.519654675737127", "module": "A5"}, {"value": "0.000253855975702815", "module": "B1"}, {"value": "0.289497877568362", "module": "B2"}, {"value": "0", "module": "C1"}, {"value": "0.0581394996199794", "module": "C2"}, {"value": "0", "module": "C3"}, {"value": "0.301101979119482", "module": "C4"}, {"value": "0.052717966155376", "module": "D"}]}}, {"referenceToLCIAMethodDataSet": {"shortDescription": [{"value": "Global Warming Potential fossil fuels (GWP-fossil)", "lang": "en"}, {"value": "Globales Erwärmungspotenzial fossil (GWP-fossil)", "lang": "de"}], "type": "LCIA method data set", "refObjectId": "5f635281-343e-44fb-83df-1971b155e6b6", "uri": "../lciamethods/5f635281-343e-44fb-83df-1971b155e6b6.xml"}, "other": {"anies": [{"name": "referenceToUnitGroupDataSet", "value": {"shortDescription": [{"value": "kg CO_(2) eq", "lang": "en"}], "type": "unit group data set", "refObjectId": "1ebf3012-d0db-4de2-aefd-ef30cedb0be1", "uri": "../unitgroups/1ebf3012-d0db-4de2-aefd-ef30cedb0be1.xml"}}, {"value": "8.14663438672801", "module": "A1-A3"}, {"value": "0.266590591615478", "module": "A4"}, {"value": "0.523781751813389", "module": "A5"}, {"value": "0.000253855975702815", "module": "B1"}, {"value": "0.286384754417568", "module": "B2"}, {"value": "0", "module": "C1"}, {"value": "0.0578965973408399", "module": "C2"}, {"value": "0", "module": "C3"}, {"value": "0.304191392137922", "module": "C4"}, {"value": "0.0484373384454423", "module": "D"}]}}, {"referenceToLCIAMethodDataSet": {"shortDescription": [{"value": "Global Warming Potential biogenic (GWP-biogenic)", "lang": "en"}, {"value": "Globales Erwärmungspotenzial biogen (GWP-biogenic)", "lang": "de"}], "type": "LCIA method data set", "refObjectId": "2356e1ab-0185-4db5-86e5-16de51c7485c", "uri": "../lciamethods/2356e1ab-0185-4db5-86e5-16de51c7485c.xml"}, "other": {"anies": [{"name": "referenceToUnitGroupDataSet", "value": {"shortDescription": [{"value": "kg CO_(2) eq", "lang": "en"}], "type": "unit group data set", "refObjectId": "1ebf3012-d0db-4de2-aefd-ef30cedb0be1", "uri": "../unitgroups/1ebf3012-d0db-4de2-aefd-ef30cedb0be1.xml"}}, {"value": "-0.340952030490461", "module": "A1-A3"}, {"value": "-0.000368342466600402", "module": "A4"}, {"value": "-0.00435197041872833", "module": "A5"}, {"value": "0", "module": "B1"}, {"value": "0.00305255201465734", "module": "B2"}, {"value": "0", "module": "C1"}, {"value": "-7.9994478961413E-05", "module": "C2"}, {"value": "0", "module": "C3"}, {"value": "-0.00323750503972626", "module": "C4"}, {"value": "0.00424302570642414", "module": "D"}]}}, {"referenceToLCIAMethodDataSet": {"shortDescription": [{"value": "Global Warming Potential luluc (GWP-luluc)", "lang": "en"}, {"value": "Globales Erwärmungspotenzial luluc (GWP-luluc)", "lang": "de"}], "type": "LCIA method data set", "refObjectId": "4331bbdb-978a-490d-8707-eeb047f01a55", "uri": "../lciamethods/4331bbdb-978a-490d-8707-eeb047f01a55.xml"}, "other": {"anies": [{"name": "referenceToUnitGroupDataSet", "value": {"shortDescription": [{"value": "kg CO_(2) eq", "lang": "en"}], "type": "unit group data set", "refObjectId": "1ebf3012-d0db-4de2-aefd-ef30cedb0be1", "uri": "../unitgroups/1ebf3012-d0db-4de2-aefd-ef30cedb0be1.xml"}}, {"value": "0.00204353820159184", "module": "A1-A3"}, {"value": "0.00148680996339162", "module": "A4"}, {"value": "0.000224894342466125", "module": "A5"}, {"value": "0", "module": "B1"}, {"value": "6.05711361367548E-05", "module": "B2"}, {"value": "0", "module": "C1"}, {"value": "0.00032289675810088", "module": "C2"}, {"value": "0", "module": "C3"}, {"value": "0.000148092021285796", "module": "C4"}, {"value": "3.7602003509231E-05", "module": "D"}]}}, {"referenceToLCIAMethodDataSet": {"shortDescription": [{"value": "Depletion potential of the stratospheric ozone layer (ODP)", "lang": "en"}, {"value": "Abbau Potential der stratosphärischen Ozonschicht (ODP)", "lang": "de"}], "type": "LCIA method data set", "refObjectId": "b5c629d6-def3-11e6-bf01-fe55135034f3", "uri": "../lciamethods/b5c629d6-def3-11e6-bf01-fe55135034f3.xml"}, "other": {"anies": [{"name": "referenceToUnitGroupDataSet", "value": {"shortDescription": [{"value": "kg CFC11 eq", "lang": "en"}], "type": "unit group data set", "refObjectId": "d9e957c9-7309-4474-bf3a-7777df6c4e5b", "uri": "../unitgroups/d9e957c9-7309-4474-bf3a-7777df6c4e5b.xml"}}, {"value": "8.27876662482156E-09", "module": "A1-A3"}, {"value": "1.59773538555406E-14", "module": "A4"}, {"value": "4.35955491412312E-10", "module": "A5"}, {"value": "0", "module": "B1"}, {"value": "4.18789260002589E-12", "module": "B2"}, {"value": "0", "module": "C1"}, {"value": "3.46986897452325E-15", "module": "C2"}, {"value": "0", "module": "C3"}, {"value": "4.0858930549209E-13", "module": "C4"}, {"value": "1.53467696005236E-13", "module": "D"}]}}, {"referenceToLCIAMethodDataSet": {"shortDescription": [{"value": "Acidification potential of land and water (AP)", "lang": "en"}, {"value": "Versauerungspotenzial von Boden und Wasser (AP)", "lang": "de"}], "type": "LCIA method data set", "refObjectId": "b5c611c6-def3-11e6-bf01-fe55135034f3", "uri": "../lciamethods/b5c611c6-def3-11e6-bf01-fe55135034f3.xml"}, "other": {"anies": [{"name": "referenceToUnitGroupDataSet", "value": {"shortDescription": [{"value": "mol H^(+) eq", "lang": "en"}], "type": "unit group data set", "refObjectId": "42e089ac-92bf-4bf2-8ca1-5fc40d18f2ed", "uri": "../unitgroups/42e089ac-92bf-4bf2-8ca1-5fc40d18f2ed.xml"}}, {"value": "0.0199043824383132", "module": "A1-A3"}, {"value": "0.00027477555303521", "module": "A4"}, {"value": "0.00146770558406643", "module": "A5"}, {"value": "0", "module": "B1"}, {"value": "0.000628716165609844", "module": "B2"}, {"value": "0", "module": "C1"}, {"value": "5.96741597547906E-05", "module": "C2"}, {"value": "0", "module": "C3"}, {"value": "0.000901547590366061", "module": "C4"}, {"value": "0.000112575693477815", "module": "D"}]}}, {"referenceToLCIAMethodDataSet": {"shortDescription": [{"value": "Eutrophication potential aquatic freshwater (EP-freshwater)", "lang": "en"}, {"value": "Eutrophierungspotenzial Süßwasser (EP-freshwater)", "lang": "de"}], "type": "LCIA method data set", "refObjectId": "b53ec18f-7377-4ad3-86eb-cc3f4f276b2b", "uri": "../lciamethods/b53ec18f-7377-4ad3-86eb-cc3f4f276b2b.xml"}, "other": {"anies": [{"name": "referenceToUnitGroupDataSet", "value": {"shortDescription": [{"value": "kg P eq", "lang": "en"}], "type": "unit group data set", "refObjectId": "0429039d-a61d-4590-ba67-aa4a20a810a1", "uri": "../unitgroups/0429039d-a61d-4590-ba67-aa4a20a810a1.xml"}}, {"value": "2.11599184857019E-05", "module": "A1-A3"}, {"value": "7.96029683502156E-07", "module": "A4"}, {"value": "1.60288896581477E-05", "module": "A5"}, {"value": "0", "module": "B1"}, {"value": "1.39786623985171E-06", "module": "B2"}, {"value": "0", "module": "C1"}, {"value": "1.72877106344231E-07", "module": "C2"}, {"value": "0", "module": "C3"}, {"value": "5.67836980144691E-05", "module": "C4"}, {"value": "7.44179418209234E-08", "module": "D"}]}}, {"referenceToLCIAMethodDataSet": {"shortDescription": [{"value": "Eutrophication potential aquatic marine (EP-marine)", "lang": "en"}, {"value": "Eutrophierungspotenzial Salzwasser (EP-marine)", "lang": "de"}], "type": "LCIA method data set", "refObjectId": "b5c619fa-def3-11e6-bf01-fe55135034f3", "uri": "../lciamethods/b5c619fa-def3-11e6-bf01-fe55135034f3.xml"}, "other": {"anies": [{"name": "referenceToUnitGroupDataSet", "value": {"shortDescription": [{"value": "kg N eq", "lang": "en"}], "type": "unit group data set", "refObjectId": "d05bb823-ecdf-4686-8c40-bf1d9257859f", "uri": "../unitgroups/d05bb823-ecdf-4686-8c40-bf1d9257859f.xml"}}, {"value": "0.00519790263958554", "module": "A1-A3"}, {"value": "8.98955626749993E-05", "module": "A4"}, {"value": "0.000349631418034669", "module": "A5"}, {"value": "0", "module": "B1"}, {"value": "0.000143247000807076", "module": "B2"}, {"value": "0", "module": "C1"}, {"value": "1.95229965295613E-05", "module": "C2"}, {"value": "0", "module": "C3"}, {"value": "0.000199455568671138", "module": "C4"}, {"value": "4.15854643138221E-05", "module": "D"}]}}, {"referenceToLCIAMethodDataSet": {"shortDescription": [{"value": "Eutrophication potential terrestrial (EP-terrestrial)", "lang": "en"}, {"value": "Eutrophierungspotenzial Land (EP-terrestrial)", "lang": "de"}], "type": "LCIA method data set", "refObjectId": "b5c614d2-def3-11e6-bf01-fe55135034f3", "uri": "../lciamethods/b5c614d2-def3-11e6-bf01-fe55135034f3.xml"}, "other": {"anies": [{"name": "referenceToUnitGroupDataSet", "value": {"shortDescription": [{"value": "mol N eq", "lang": "en"}], "type": "unit group data set", "refObjectId": "71b4d617-0ec9-4d3f-b65e-e438940c2401", "uri": "../unitgroups/71b4d617-0ec9-4d3f-b65e-e438940c2401.xml"}}, {"value": "0.0511046044250909", "module": "A1-A3"}, {"value": "0.00107007241315647", "module": "A4"}, {"value": "0.00415862107932576", "module": "A5"}, {"value": "0", "module": "B1"}, {"value": "0.00148078726506181", "module": "B2"}, {"value": "0", "module": "C1"}, {"value": "0.000232392115770615", "module": "C2"}, {"value": "0", "module": "C3"}, {"value": "0.00218755018459081", "module": "C4"}, {"value": "0.000391421547500849", "module": "D"}]}}, {"referenceToLCIAMethodDataSet": {"shortDescription": [{"value": "Formation potential of tropospheric ozone photochemical oxidants (POCP)", "lang": "en"}, {"value": "Bildungspotential für troposphärisches Ozon (POCP)", "lang": "de"}], "type": "LCIA method data set", "refObjectId": "b5c610fe-def3-11e6-bf01-fe55135034f3", "uri": "../lciamethods/b5c610fe-def3-11e6-bf01-fe55135034f3.xml"}, "other": {"anies": [{"name": "referenceToUnitGroupDataSet", "value": {"shortDescription": [{"value": "kg NMVOC eq", "lang": "en"}], "type": "unit group data set", "refObjectId": "d27c25f8-fbc1-44c6-b47b-4adbae4199c6", "uri": "../unitgroups/d27c25f8-fbc1-44c6-b47b-4adbae4199c6.xml"}}, {"value": "0.0171131798821165", "module": "A1-A3"}, {"value": "0.000242089970770008", "module": "A4"}, {"value": "0.0012378247347601", "module": "A5"}, {"value": "1.41031097612675E-05", "module": "B1"}, {"value": "0.000381501967813061", "module": "B2"}, {"value": "0", "module": "C1"}, {"value": "5.25756947122251E-05", "module": "C2"}, {"value": "0", "module": "C3"}, {"value": "0.000641644004139711", "module": "C4"}, {"value": "0.000119539730204543", "module": "D"}]}}, {"referenceToLCIAMethodDataSet": {"shortDescription": [{"value": "Abiotic depletion potential for non fossil resources (ADPE)", "lang": "en"}, {"value": "Potenzial für den abiotischen Abbau nicht fossiler Ressourcen (ADPE)", "lang": "de"}], "type": "LCIA method data set", "refObjectId": "b2ad6494-c78d-11e6-9d9d-cec0c932ce01", "uri": "../lciamethods/b2ad6494-c78d-11e6-9d9d-cec0c932ce01.xml"}, "other": {"anies": [{"name": "referenceToUnitGroupDataSet", "value": {"shortDescription": [{"value": "kg Sb eq", "lang": "en"}], "type": "unit group data set", "refObjectId": "54ccd2d9-a32a-4fc2-923d-f2c8c93e89d4", "uri": "../unitgroups/54ccd2d9-a32a-4fc2-923d-f2c8c93e89d4.xml"}}, {"value": "2.58357966827462E-06", "module": "A1-A3"}, {"value": "2.22937466554834E-08", "module": "A4"}, {"value": "1.61563011693434E-07", "module": "A5"}, {"value": "0", "module": "B1"}, {"value": "7.79609995435807E-08", "module": "B2"}, {"value": "0", "module": "C1"}, {"value": "4.84162650118174E-09", "module": "C2"}, {"value": "0", "module": "C3"}, {"value": "2.10953548101238E-08", "module": "C4"}, {"value": "3.69132059529696E-09", "module": "D"}]}}, {"referenceToLCIAMethodDataSet": {"shortDescription": [{"value": "Abiotic depletion potential for fossil resources (ADPF)", "lang": "en"}, {"value": "Potenzial für den abiotischen Abbau fossiler Brennstoffe (ADPF)", "lang": "de"}], "type": "LCIA method data set", "refObjectId": "b2ad6110-c78d-11e6-9d9d-cec0c932ce01", "uri": "../lciamethods/b2ad6110-c78d-11e6-9d9d-cec0c932ce01.xml"}, "other": {"anies": [{"name": "referenceToUnitGroupDataSet", "value": {"shortDescription": [{"value": "MJ", "lang": "en"}], "type": "unit group data set", "refObjectId": "93a60a57-a3c8-11da-a746-0800200c9a66", "uri": "../unitgroups/93a60a57-a3c8-11da-a746-0800200c9a66.xml"}}, {"value": "178.616061221312", "module": "A1-A3"}, {"value": "3.56380841828827", "module": "A4"}, {"value": "10.8272651887749", "module": "A5"}, {"value": "0", "module": "B1"}, {"value": "5.19171180454845", "module": "B2"}, {"value": "0", "module": "C1"}, {"value": "0.77396722721235", "module": "C2"}, {"value": "0", "module": "C3"}, {"value": "4.31663328244165", "module": "C4"}, {"value": "0.854957588276585", "module": "D"}]}}, {"referenceToLCIAMethodDataSet": {"shortDescription": [{"value": "Water use (WDP)", "lang": "en"}, {"value": "Wassernutzung (WDP)", "lang": "de"}], "type": "LCIA method data set", "refObjectId": "b2ad66ce-c78d-11e6-9d9d-cec0c932ce01", "uri": "../lciamethods/b2ad66ce-c78d-11e6-9d9d-cec0c932ce01.xml"}, "other": {"anies": [{"name": "referenceToUnitGroupDataSet", "value": {"shortDescription": [{"value": "m^(3) world eq deprived", "lang": "en"}], "type": "unit group data set", "refObjectId": "6ae2df01-888e-46c8-b17d-49fa3869b476", "uri": "../unitgroups/6ae2df01-888e-46c8-b17d-49fa3869b476.xml"}}, {"value": "0.774071502710961", "module": "A1-A3"}, {"value": "0.00239208870294757", "module": "A4"}, {"value": "0.110556646978596", "module": "A5"}, {"value": "0", "module": "B1"}, {"value": "0.0653913269118636", "module": "B2"}, {"value": "0", "module": "C1"}, {"value": "0.000519499940335053", "module": "C2"}, {"value": "0", "module": "C3"}, {"value": "-0.00299899774377872", "module": "C4"}, {"value": "-0.00226654349486003", "module": "D"}]}}, {"referenceToLCIAMethodDataSet": {"shortDescription": [{"value": "Incidence of disease due to PM emissions (PM)", "lang": "en"}, {"value": "Auftreten von Krankheiten aufgrund von Feinstaubemissionen (PM)", "lang": "de"}], "type": "LCIA method data set", "refObjectId": "b5c602c6-def3-11e6-bf01-fe55135034f3", "uri": "../lciamethods/b5c602c6-def3-11e6-bf01-fe55135034f3.xml"}, "other": {"anies": [{"name": "referenceToUnitGroupDataSet", "value": {"shortDescription": [{"value": "Disease incidence", "lang": "en"}], "type": "unit group data set", "refObjectId": "3883559b-648f-4afc-8ba2-0bd24f3affa3", "uri": "../unitgroups/3883559b-648f-4afc-8ba2-0bd24f3affa3.xml"}}, {"value": "1.79083041025473E-07", "module": "A1-A3"}, {"value": "1.58635155886015E-09", "module": "A4"}, {"value": "1.43283847562554E-08", "module": "A5"}, {"value": "0", "module": "B1"}, {"value": "5.21482253511121E-09", "module": "B2"}, {"value": "0", "module": "C1"}, {"value": "3.44514624044996E-10", "module": "C2"}, {"value": "0", "module": "C3"}, {"value": "8.6643403303776E-09", "module": "C4"}, {"value": "1.8278294529491E-08", "module": "D"}]}}, {"referenceToLCIAMethodDataSet": {"shortDescription": [{"value": "Human exposure efficiency relative to U235 (IR)", "lang": "en"}, {"value": "Wirkung durch Exposition des Menschen mit U235 (IR)", "lang": "de"}], "type": "LCIA method data set", "refObjectId": "b5c632be-def3-11e6-bf01-fe55135034f3", "uri": "../lciamethods/b5c632be-def3-11e6-bf01-fe55135034f3.xml"}, "other": {"anies": [{"name": "referenceToUnitGroupDataSet", "value": {"shortDescription": [{"value": "kBq U235 eq", "lang": "en"}], "type": "unit group data set", "refObjectId": "456b05bf-1415-44a9-9993-02452f554c09", "uri": "../unitgroups/456b05bf-1415-44a9-9993-02452f554c09.xml"}}, {"value": "0.424552211572491", "module": "A1-A3"}, {"value": "0.000644773082463668", "module": "A4"}, {"value": "0.0249574498311058", "module": "A5"}, {"value": "0", "module": "B1"}, {"value": "0.140562657769239", "module": "B2"}, {"value": "0", "module": "C1"}, {"value": "0.000140028075654879", "module": "C2"}, {"value": "0", "module": "C3"}, {"value": "0.007828859763204", "module": "C4"}, {"value": "0.00366018783759183", "module": "D"}]}}, {"referenceToLCIAMethodDataSet": {"shortDescription": [{"value": "Comparative toxic unit for ecosystems (ETP-fw)", "lang": "en"}, {"value": "Toxizitätsvergleichseinheit für Ökosysteme (ETP-fw)", "lang": "de"}], "type": "LCIA method data set", "refObjectId": "ee1082d1-b0f7-43ca-a1f0-21e2a4a74511", "uri": "../lciamethods/ee1082d1-b0f7-43ca-a1f0-21e2a4a74511.xml"}, "other": {"anies": [{"name": "referenceToUnitGroupDataSet", "value": {"shortDescription": [{"value": "CTUe", "lang": "en"}], "type": "unit group data set", "refObjectId": "aa959ded-f1eb-4efb-9c5c-2d60be36b3e6", "uri": "../unitgroups/aa959ded-f1eb-4efb-9c5c-2d60be36b3e6.xml"}}, {"value": "93.4054417655234", "module": "A1-A3"}, {"value": "2.47418743031284", "module": "A4"}, {"value": "5.99463152803912", "module": "A5"}, {"value": "0.000115063371682035", "module": "B1"}, {"value": "2.34808205613559", "module": "B2"}, {"value": "0", "module": "C1"}, {"value": "0.537329665426472", "module": "C2"}, {"value": "0", "module": "C3"}, {"value": "4.22422977915702", "module": "C4"}, {"value": "0.380061996107691", "module": "D"}]}}, {"referenceToLCIAMethodDataSet": {"shortDescription": [{"value": "Comparative toxic unit for humans (carcinogenic) (HTP-c)", "lang": "en"}, {"value": "Toxizitätsvergleichseinheit für Menschen (krebserregend) (HTP-c)", "lang": "de"}], "type": "LCIA method data set", "refObjectId": "2299222a-bbd8-474f-9d4f-4dd1f18aea7c", "uri": "../lciamethods/2299222a-bbd8-474f-9d4f-4dd1f18aea7c.xml"}, "other": {"anies": [{"name": "referenceToUnitGroupDataSet", "value": {"shortDescription": [{"value": "CTUh", "lang": "en"}], "type": "unit group data set", "refObjectId": "d4c9523e-2d7e-49fd-8469-998f547d3a70", "uri": "../unitgroups/d4c9523e-2d7e-49fd-8469-998f547d3a70.xml"}}, {"value": "2.51708524080177E-09", "module": "A1-A3"}, {"value": "4.98695299960011E-11", "module": "A4"}, {"value": "1.7050826892691E-10", "module": "A5"}, {"value": "0", "module": "B1"}, {"value": "6.7868087675296E-11", "module": "B2"}, {"value": "0", "module": "C1"}, {"value": "1.08303750716002E-11", "module": "C2"}, {"value": "0", "module": "C3"}, {"value": "1.89677105367916E-10", "module": "C4"}, {"value": "1.31581588407124E-11", "module": "D"}]}}, {"referenceToLCIAMethodDataSet": {"shortDescription": [{"value": "Comparative toxic unit for humans (noncarcinogenic) (HTP-nc)", "lang": "en"}, {"value": "Toxizitätsvergleichseinheit für Menschen (nicht krebserregend) (HTP-nc)", "lang": "de"}], "type": "LCIA method data set", "refObjectId": "3af763a5-b7a1-48c9-9cee-1f223481fcef", "uri": "../lciamethods/3af763a5-b7a1-48c9-9cee-1f223481fcef.xml"}, "other": {"anies": [{"name": "referenceToUnitGroupDataSet", "value": {"shortDescription": [{"value": "CTUh", "lang": "en"}], "type": "unit group data set", "refObjectId": "d4c9523e-2d7e-49fd-8469-998f547d3a70", "uri": "../unitgroups/d4c9523e-2d7e-49fd-8469-998f547d3a70.xml"}}, {"value": "1.14232520229941E-07", "module": "A1-A3"}, {"value": "2.5877775111496E-09", "module": "A4"}, {"value": "8.34887199401142E-09", "module": "A5"}, {"value": "3.06571599593442E-12", "module": "B1"}, {"value": "2.65484681526225E-09", "module": "B2"}, {"value": "0", "module": "C1"}, {"value": "5.61998499882582E-10", "module": "C2"}, {"value": "0", "module": "C3"}, {"value": "1.58972390231557E-08", "module": "C4"}, {"value": "5.37279576024953E-10", "module": "D"}]}}, {"referenceToLCIAMethodDataSet": {"shortDescription": [{"value": "Soil quality index (SQP)", "lang": "en"}, {"value": "Bodenqualitätsindex (SQP)", "lang": "de"}], "type": "LCIA method data set", "refObjectId": "b2ad6890-c78d-11e6-9d9d-cec0c932ce01", "uri": "../lciamethods/b2ad6890-c78d-11e6-9d9d-cec0c932ce01.xml"}, "other": {"anies": [{"name": "referenceToUnitGroupDataSet", "value": {"shortDescription": [{"value": "SQP", "lang": "en"}], "type": "unit group data set", "refObjectId": "f130951c-e67f-4f7f-8dd4-665de3974e18", "uri": "../unitgroups/f130951c-e67f-4f7f-8dd4-665de3974e18.xml"}}, {"value": "11.8294832925296", "module": "A1-A3"}, {"value": "1.22630070302387", "module": "A4"}, {"value": "11.0500742154391", "module": "A5"}, {"value": "0", "module": "B1"}, {"value": "1.87183086256323", "module": "B2"}, {"value": "0", "module": "C1"}, {"value": "0.266320868983133", "module": "C2"}, {"value": "0", "module": "C3"}, {"value": "0.310580896913008", "module": "C4"}, {"value": "-0.506005651600284", "module": "D"}]}}]}, "otherAttributes": {"{http://www.indata.network/EPD/2019}epd-version": "1.2"}, "version": "1.1", "locations": "../ILCDLocations.xml"}