{"processInformation": {"dataSetInformation": {"UUID": "5a580331-75c4-43c8-b732-19fc1cc8e97a", "name": {"baseName": [{"value": "EGGER DHF", "lang": "de"}, {"value": "EGGER DHF", "lang": "en"}], "functionalUnitFlowProperties": [{"lang": "de"}]}, "classificationInformation": {"classification": [{"class": [{"value": "Holz", "level": 0, "classId": "3"}, {"value": "Holzwerkstoffe", "level": 1, "classId": "3.2"}, {"value": "Holzfaserplatten", "level": 2, "classId": "3.2.07"}], "name": "OEKOBAU.DAT"}, {"class": [{"value": "02 Bauprodukte", "level": 0}, {"value": "Holzwerkstoffe", "level": 1}, {"value": "Holzwerkstoffe", "level": 2}], "name": "IBUCategories"}]}, "generalComment": [{"value": "EGGER DHF-Platten sind kunstharzgebundene mitteldichte Holzfaserplatten gemäß EN 622-5 (Plattentyp MDF.RWH), die im Trockenverfahren hergestellt werden. Sie basieren hauptsächlich auf Fasern aus Nadelholz. Die Holzwerkstoffplatten sind im Kantenbereich mit Nut- und Feder-Profil versehen. Die Durchschnittsdaten spiegeln die für die DHF-Platten spezifische Produktionssituation für eine Dichte von 615 kg/m³ wider.", "lang": "de"}, {"value": "EGGER\nDHF boards are synthetic resin-bonded medium-density wood fibre boards\naccording to EN 622-5 (board type MDF.RWH), which are manufactured in a\ndry process. They are mainly based on fibres from softwood. The wood-based\npanels are fitted with tongue and groove profiles in the edge area. The average\ndata reflects the specific production situation for DHF boards for a density of\n615 kg/m³.", "lang": "en"}]}, "quantitativeReference": {"referenceToReferenceFlow": [0]}, "time": {"referenceYear": 2021, "dataSetValidUntil": 2027, "other": {"anies": [{"name": "publicationDateOfEPD", "value": 1618790400000}]}}, "geography": {"locationOfOperationSupplyOrProduction": {"location": "DE"}}, "technology": {"technologyDescriptionAndIncludedProcesses": [{"value": "Sägewerksrestholz bzw. entrindete Holzstämme werden auf eine definierte Größe zerkleinert und anschließend in einem Kocher bei hohem Druck gekocht und über Mahlscheiben zu Holzfasern zerrieben. Diese Holzfasern werden beleimt und in einer kontinuierlich arbeitenden Streustation zu einem Endlos-Faserkuchen gestreut. Dieser Kuchen wird ebenso endlos durch eine kontinuierliche Heißpresse gefördert und dabei immer weiter auf die gewünschte Enddicke verdichtet. Nach der Presse wird der endlose Plattenstrang auf das erforderliche Rohplattenmaß zugeschnitten und in großen Kühlsternwendern auf Raumtemperatur gekühlt. Die Platten werden anschließend in der Endfertigung auf das Plattenendmaß zugeschnitten und mit Nut- und Feder-Profil versehen, verpackt und für den Versand gelagert. Die Produktion umfasst die folgenden Prozessschritte: 1. Entrindung der Stämme 2. Zerspanung des Holzes zu Spänen und Hackschnitzel 3. Kochen der Späne und Hackschnitzel 4. Zerfaserung im Refiner 5. Trocknung der Fasern auf ca. 2-3 % Restfeuchte 6. Beleimung der Fasern mit Harzen 7. Streuung der beleimten Fasern auf ein Formband 8. Verpressen der Fasermatte in einer kontinuierlich arbeitenden Heißpresse 9. Aufteilen und Besäumen des Faserstranges zu Rohplattenformaten 10. Auskühlen der Rohplatten in Kühlsternwender 11. Abstapelung zu Großstapeln 12. Endfertigung / Nut-und Feder-Anlage Alle während der Produktion anfallenden Reste (Besäum- und Fräsreste) werden ausnahmslos einer thermischen Verwertung zugeführt. \nTechnische Daten: \nFür EGGER DHF-Platten mit CE-Kennzeichnung nach EN 13986:2004+A1:2015 bzw. EN 14964:2006 liegt eine Leistungserklärung (DoP) mit den maßgebenden Daten vor unter: www.egger.com. \nDeklarierte Einheit: \nDie vorliegende Umwelt-Produktdeklaration bezieht sich auf eine deklarierte Einheit von 1 m³ EGGER DHF-Platte mit einer durchschnittlichen Rohdichte von 615 kg/m³ und einer Auslieferungsfeuchte von 7,5 %.", "lang": "de"}, {"value": "Sawmill residues or debarked logs are crushed to a defined size and then cooked in a high pressure cooker and turned into wood fibres with grinding discs. These wood fibres are coated with glue and strewn in a continuously working dispersing station to form a continuous fibre cake. This cake is then continuously transported through a continuous hot press, and thus constantly compressed to the desired final thickness. After the press, the continuous board strand is cut to the required raw board size and cooled in large star coolers to room temperature. The boards are then cut to final size during finishing and fitted with tongue and groove profiles, packaged, and stored for shipping. The production includes the following process stages: 1. Peeling logs 2. Chipping the wood to produce chips and wood chips 3. Cooking the chips and wood chips 4. Defibration in the refiner 5. Drying the fibres to approximately 2 – 3 % residual moisture 6. Application of resin to the fibres 7. Spreading the glue-coated fibres onto a forming belt 8. Compression of the fibre mat in a hot press that works continuously 9. Cutting and trimming the fibre strand into rawboard formats 10. Cooling the rawboards in star coolers 11. Piling into large stacks 12. Finishing / tongue and groove line All waste generated in the course of production (trimming and milling waste) is used thermally with no exceptions. The Wismar plant is certified with a quality management system according to ISO 9001. \nTechnical data: \nA declaration of performance (DoP) with\nrelevant data for EGGER DHF boards with CE marking according to EN 13986:2004+A1:2015\nand EN 14964:2006 are available at www.egger.com. \nDeclared unit: \nThis environmental product declaration is\nbased on a declared unit of 1 m³ EGGER DHF board with an average raw density of\n615 kg/m³ and a delivery moisture of approximately 7.5 %.", "lang": "en"}], "technologicalApplicability": [{"value": "EGGER DHF-Platten werden vorwiegend als diffusionsoffene, wärmedämmende und zum Teil mittragende Beplankung in Dach und Wand eingesetzt. Sie erfüllen die Anforderungen als Unterdeckung des Typs UDP-A gemäß Richtlinie des Zentralverbandes des Deutschen Dachdeckerhandwerks (ZVDH). \n\nDHF-Platten können als mittragende Außenbeplankung von Wänden und Dächern in den Nutzungsklassen 1 und 2 nach EN 1995-1-1 unter Berücksichtigung der DIN 68800-2 eingesetzt werden.\nZusätzlich zu den zuvor genannten Anwendungsbestimmungen sind die jeweiligen nationalen Vorschriften zu beachten.", "lang": "de"}, {"value": "EGGER DHF boards are mainly used as vapour\npermeable, heat-insulating and partly load-bearing cladding in roofs and walls.\nThey meet the requirements as sub-roofing of type UDP-A according to the\nguideline of the Central Association of German Roofers (ZVDH). \nDHF boards can be used as load-bearing external\ncladding for walls and roofs in service classes 1 and 2 according to EN\n1995-1-1, taking into account DIN 68800-2. \n\nIn addition to the aforementioned\napplication regulations, the respective national regulations must be\nobserved.", "lang": "en"}]}}, "modellingAndValidation": {"LCIMethodAndAllocation": {"typeOfDataSet": "EPD", "referenceToLCAMethodDetails": [{"shortDescription": [{"value": "Holzwerkstoffe.pdf", "lang": "de"}], "type": "source data set", "refObjectId": "8bb66ccf-ac3e-4915-96a0-a425c1a67a2b"}], "other": {"anies": [{"name": "subType", "value": "specific dataset"}]}}, "dataSourcesTreatmentAndRepresentativeness": {"referenceToDataSource": [{"shortDescription": [{"value": "GaBi Database (all versions)", "lang": "de"}], "type": "source data set", "refObjectId": "28d74cc0-db8b-4d7e-bc44-5f6d56ce0c4a"}, {"shortDescription": [{"value": "GaBi database SP40 2020", "lang": "de"}], "type": "source data set", "refObjectId": "0115289e-52f0-4920-bc7e-57b1c96aec8d"}], "useAdviceForDataSet": [{"value": "Gültigkeitsbereich: \nDieses Dokument bezieht sich auf DHF-Platten, welche in folgendem Werk hergestellt werden:\n\nEgger Holzwerkstoffe Wismar GmbH & Co. KG\nAm Haffeld 1, 23970 Wismar, Deutschland \nSystemgrenze: \nDie Ökobilanz der EGGER DHF beinhaltet eine cradle-to-gate Betrachtung (Wiege bis zum Werkstor) der auftretenden Umweltwirkungen mit den Modulen C1-C4 und\nModul D (A1-A3, +C, +D). Die folgenden Lebenszyklusphasen werden in der Analyse berücksichtigt:\n\nModul A1-A3 | Produktionsstadium\n\nDas Produktionsstadium beinhaltet die\nAufwendungen der Rohstoffversorgung (Rundholz, Herstellung des Leimsystems, der\nEmulsion und des Trennmittels etc.) sowie der damit verbundenen Transporte\nbezogen auf den Produktionsstandort in Wismar. Innerhalb der Werksgrenzen werden\ndie DHF-Plattenproduktion, die Endfertigung und das Ausgangslager inklusive der\nVerpackung des Produkts berücksichtigt. Der Großteil der eingesetzten elektrischen Energie wird vom deutschen Stromnetz\nbezogen. Im eigenen\nBiomasse-Kraftwerk wird sowohl internes Restholz als auch extern bezogenes\nAltholz verwertet. Die Systemgrenze für in der Produktion verwendetes Altholz\nwird nach dem Sortieren und Hacken gesetzt. Dabei wird angenommen, dass das\nEnde der Abfalleigenschaft erreicht ist. Hier gilt die nach EN\n15804 definierte Systemgrenze für\nSekundärrohstoffe.\n\n\nModul C1 | Rückbau / Abriss\nFür die DHF-Platten wurde ein manueller Ausbau angenommen. Die damit verbundenen Aufwände sind vernachlässigbar, wodurch keine Umweltwirkungen aus dem Rückbau der Produkte deklariert werden.\n\n\nModul C2 | Transport zur Abfallbehandlung\nModul C2 beinhaltet den Transport zur Abfallbehandlung. Dazu wird der Transport via LKW über 50 km Transportdistanz als repräsentatives Szenario angesetzt.\n\nModul C3 | Abfallbehandlung\n\nDas Holzprodukt und mit ihm die materialinhärenten Eigenschaften verlassen das Produktsystem als Sekundärbrennstoff in Modul C3. Darüber hinaus wird das Hacken nach Ausbau des Produktes betrachtet.\n\n\nModul C4 | Beseitigung\nDas angesetzte Szenario deklariert die energetische Verwertung der Holzprodukte, wodurch keine Umweltauswirkungen aus der Abfallbehandlung der Produkte in C4 zu erwarten sind.\n\nModul D | Gutschriften und Lasten außerhalb der\nSystemgrenzen \n\nIn Modul D wird die energetische Verwertung des\nProduktes am Lebensende inklusive den entsprechenden energetischen Substitutionspotenzialen\nin Form eines europäischen Durchschnittsszenarios beschrieben.", "lang": "de"}, {"value": "Scope: \nThis document refers to DHF boards, which\nare manufactured in the following plant:\n\n\n\nEgger Holzwerkstoffe Wismar GmbH\n& Co. KG\n\n\nAm Haffeld 1, 23970 Wismar, Germany \nSystem boundary: \nThe LCA of the EGGER DHF includes a\ncradle-to-gate consideration of the occurring environmental impact with the\nmodules C1-C4 and module D (A1-A3, +C, +D). The following life cycle phases are\ntaken into account in the analysis:\n\n\n\nModule A1– A3 | Production stage \n\n\nThe production stage includes the cost\nof raw material procurement (roundwood, producing the glue system, the emulsion\nand the separating agent, etc.), as well as related transport relative to the\nproduction plant in Wismar. Within the plant boundaries, DHF board production,\nfinishing and the outgoing warehouse including the packaging of the product are\ntaken into account. The majority of the electrical energy used is obtained from\nthe German power grid. Both internal wood waste and scrap wood sourced\nexternally are used in the in-house biomass power plant. The system\nboundary for the scrap wood used in the production is set after sorting and\nchopping. It is assumed that the end of the waste status has been reached. The\nsystem boundary for secondary raw materials according to EN 15804\napplies.\n\n\n\nModule C1 | Dismantling / Demolition\nManual removal was assumed for the DHF boards. The\nassociated efforts are negligible, which means that no environmental impact\nfrom the dismantling of the products is declared.\n\n\n\nModule C2 | Transport to waste\ntreatment\n\nModule C2 includes transport to waste treatment.\nFor this purpose, transport by lorry over a distance of 50 km is used as a\nrepresentative scenario.\n\n\n\nModule C3 | Waste processing\n\n\nThe wood product and with it the\nmaterial-inherent properties leave the product system as secondary fuel in\nmodule C3. Furthermore, chopping after product disassembly is also considered.\n\n\n\nModule C4 | Disposal\n\nThe scenario used declares the energy recovery of\nthe wood products, which means that no environmental impact from the waste\ntreatment of the products in C4 are to be expected.\n\n\n\nModule D | Credits and charges\noutside the system limits \n\n\nThe energy utilisation of the product\nat the end of its life cycle is described in Module D, including energetic\nsubstitution potential as a European average scenario.", "lang": "en"}], "other": {"anies": [{"name": "referenceToOriginalEPD", "value": {"shortDescription": {"value": "EGGER DHF.pdf", "defaultValue": "EGGER DHF.pdf", "lstrings": [{"lang": "de", "value": "EGGER DHF.pdf"}]}, "type": "source data set", "uuid": {"uuid": "e8f1fdc7-cc4e-474d-ad8d-73fa365f2b14"}, "refObjectId": "e8f1fdc7-cc4e-474d-ad8d-73fa365f2b14", "resourceURLs": ["https://oekobaudat.de/OEKOBAU.DAT/resource/sources/e8f1fdc7-cc4e-474d-ad8d-73fa365f2b14/EGGER_DHF_23553.pdf?version=00.02.000"]}}]}}, "validation": {"review": [{"referenceToNameOfReviewerAndInstitution": [{"shortDescription": [{"value": "Institut Bauen und Umwelt e. V.", "lang": "de"}], "type": "contact data set", "refObjectId": "d111dbec-b024-4be5-86c5-752d6eb2cf95", "uri": "../contacts/d111dbec-b024-4be5-86c5-752d6eb2cf95.xml"}], "type": "Accredited third party review"}]}, "complianceDeclarations": {"compliance": [{"referenceToComplianceSystem": {"shortDescription": [{"value": "DIN EN 15804+A2", "lang": "de"}], "type": "source data set", "refObjectId": "c0016b33-8cf7-415c-ac6e-deba0d21440d", "uri": "../sources/c0016b33-8cf7-415c-ac6e-deba0d21440d.xml"}}, {"referenceToComplianceSystem": {"shortDescription": [{"value": "ISO 14025", "lang": "de"}], "type": "source data set", "refObjectId": "4f2eb655-6e44-4874-a95a-e28f5442cd4d", "uri": "../sources/4f2eb655-6e44-4874-a95a-e28f5442cd4d.xml"}}]}}, "administrativeInformation": {"commissionerAndGoal": {"referenceToCommissioner": [{"shortDescription": [{"value": "Fritz EGGER GmbH & Co. OG", "lang": "de"}], "type": "contact data set", "refObjectId": "3ccb1a8b-2f9d-4de9-b22b-777128355981", "uri": "../contacts/3ccb1a8b-2f9d-4de9-b22b-777128355981.xml"}]}, "dataGenerator": {"referenceToPersonOrEntityGeneratingTheDataSet": [{"shortDescription": [{"value": "Daxner & Merl GmbH", "lang": "de"}], "type": "contact data set", "refObjectId": "ad8ad627-3991-42b7-a7ca-5a3fe0a34c28", "uri": "../contacts/ad8ad627-3991-42b7-a7ca-5a3fe0a34c28.xml"}]}, "dataEntryBy": {"timeStamp": 1618790400000, "referenceToDataSetFormat": [{"shortDescription": [{"value": "ILCD Format", "lang": "de"}], "type": "source data set", "refObjectId": "a97a0155-0234-4b87-b4ce-a45da52f2a40", "uri": "../sources/a97a0155-0234-4b87-b4ce-a45da52f2a40.xml"}, {"shortDescription": [{"value": "EPD-Datenformaterweiterungen v1.2", "lang": "de"}, {"value": "EPD Data Format Extensions v1.2", "lang": "en"}], "type": "source data set", "refObjectId": "a29449fd-aa2f-4de8-b5d7-4b06b43c6fde", "uri": "../sources/a29449fd-aa2f-4de8-b5d7-4b06b43c6fde.xml"}]}, "publicationAndOwnership": {"dataSetVersion": "00.05.000", "referenceToPrecedingDataSetVersion": [{"shortDescription": [{"value": "DHF-Platte", "lang": "de"}], "type": "process data set", "refObjectId": "d2ffd6b8-9d55-4824-9e1f-6a89e8087d55", "uri": "../processes/d2ffd6b8-9d55-4824-9e1f-6a89e8087d55.xml"}], "referenceToRegistrationAuthority": {"shortDescription": [{"value": "Institut Bauen und Umwelt e. V.", "lang": "de"}], "type": "contact data set", "refObjectId": "d111dbec-b024-4be5-86c5-752d6eb2cf95", "uri": "../contacts/d111dbec-b024-4be5-86c5-752d6eb2cf95.xml"}, "registrationNumber": "EPD-EGG-20200247-IBD2-DE", "referenceToOwnershipOfDataSet": {"shortDescription": [{"value": "Fritz EGGER GmbH & Co. OG", "lang": "de"}], "type": "contact data set", "refObjectId": "3ccb1a8b-2f9d-4de9-b22b-777128355981", "uri": "../contacts/3ccb1a8b-2f9d-4de9-b22b-777128355981.xml"}, "copyright": false, "licenseType": "Free of charge for all users and uses", "accessRestrictions": [{"value": "None", "lang": "en"}], "other": {"anies": [{"name": "referenceToPublisher", "value": {"shortDescription": [{"value": "Institut Bauen und Umwelt e. V.", "lang": "de"}], "type": "contact data set", "refObjectId": "d111dbec-b024-4be5-86c5-752d6eb2cf95", "uri": "../contacts/d111dbec-b024-4be5-86c5-752d6eb2cf95.xml"}}]}}}, "exchanges": {"exchange": [{"dataSetInternalID": 0, "referenceToFlowDataSet": {"shortDescription": [{"value": "DHF-Platte (DHF-Platte)", "lang": "de"}], "type": "flow data set", "refObjectId": "7d02e50e-ffb2-7aa6-3a15-e8e2607f2291", "uri": "../flows/7d02e50e-ffb2-7aa6-3a15-e8e2607f2291.xml"}, "meanAmount": 1.0, "referencesToDataSource": {}, "referenceFlow": true, "resolvedFlowVersion": "00.04.100", "resultingflowAmount": 1.0, "flowProperties": [{"name": [{"lang": "en", "value": "Volume"}, {"lang": "de", "value": "Volumen"}], "uuid": "93a60a56-a3c8-22da-a746-0800200c9a66", "referenceFlowProperty": true, "meanValue": 1.0, "referenceUnit": "m3", "unitGroupUUID": "cd950537-0a98-4044-9ba7-9f9a68d0a504"}], "materialProperties": [{"name": "gross density", "value": "615.0", "unit": "kg/m^3", "unitDescription": "kilograms per cubic metre"}], "typeOfFlow": "Product flow", "classification": {"classHierarchy": "Holz / Holzwerkstoffe / Holzfaserplatten", "name": "OEKOBAU.DAT"}}, {"dataSetInternalID": 1, "referenceToFlowDataSet": {"shortDescription": [{"value": "Erneuerbare Primärenergie als Energieträger (PERE)", "lang": "de"}, {"value": "Renewable primary energy as energy carrier (PERE)", "lang": "en"}], "type": "flow data set", "refObjectId": "20f32be5-0398-4288-9b6d-accddd195317", "uri": "../flows/20f32be5-0398-4288-9b6d-accddd195317.xml"}, "exchange direction": "INPUT", "other": {"anies": [{"name": "referenceToUnitGroupDataSet", "value": {"shortDescription": [{"value": "MJ", "lang": "de"}], "type": "unit group data set", "refObjectId": "93a60a57-a3c8-11da-a746-0800200c9a66", "uri": "../unitgroups/93a60a57-a3c8-11da-a746-0800200c9a66.xml"}}, {"value": "31916.6002038357", "module": "A1-A3"}, {"value": "0", "module": "C1"}, {"value": "1.47153800959973", "module": "C2"}, {"value": "10130.6923301902", "module": "C3"}, {"value": "0", "module": "C4"}, {"value": "-1767.6383224683", "module": "D"}]}, "resolvedFlowVersion": "38.00.000", "flowProperties": [], "typeOfFlow": "Other flow", "classification": {"classHierarchy": "Quantities", "name": "GaBiCategories"}}, {"dataSetInternalID": 2, "referenceToFlowDataSet": {"shortDescription": [{"value": "Erneuerbare Primärenergie zur stofflichen Nutzung (PERM)", "lang": "de"}, {"value": "Renewable primary energy resources as material utilization (PERM)", "lang": "en"}], "type": "flow data set", "refObjectId": "fb3ec0de-548d-4508-aea5-00b73bf6f702", "uri": "../flows/fb3ec0de-548d-4508-aea5-00b73bf6f702.xml"}, "exchange direction": "INPUT", "other": {"anies": [{"name": "referenceToUnitGroupDataSet", "value": {"shortDescription": [{"value": "MJ", "lang": "de"}], "type": "unit group data set", "refObjectId": "93a60a57-a3c8-11da-a746-0800200c9a66", "uri": "../unitgroups/93a60a57-a3c8-11da-a746-0800200c9a66.xml"}}, {"value": "10090.4955627907", "module": "A1-A3"}, {"value": "0", "module": "C1"}, {"value": "0", "module": "C2"}, {"value": "-10090.4955627907", "module": "C3"}, {"value": "0", "module": "C4"}, {"value": "0", "module": "D"}]}, "resolvedFlowVersion": "38.00.000", "flowProperties": [], "typeOfFlow": "Other flow", "classification": {"classHierarchy": "Quantities", "name": "GaBiCategories"}}, {"dataSetInternalID": 3, "referenceToFlowDataSet": {"shortDescription": [{"value": "Total erneuerbare Primärenergie (PERT)", "lang": "de"}, {"value": "Total use of renewable primary energy resources (PERT)", "lang": "en"}], "type": "flow data set", "refObjectId": "53f97275-fa8a-4cdd-9024-65936002acd0", "uri": "../flows/53f97275-fa8a-4cdd-9024-65936002acd0.xml"}, "exchange direction": "INPUT", "other": {"anies": [{"name": "referenceToUnitGroupDataSet", "value": {"shortDescription": [{"value": "MJ", "lang": "de"}], "type": "unit group data set", "refObjectId": "93a60a57-a3c8-11da-a746-0800200c9a66", "uri": "../unitgroups/93a60a57-a3c8-11da-a746-0800200c9a66.xml"}}, {"value": "42007.0957666264", "module": "A1-A3"}, {"value": "0", "module": "C1"}, {"value": "1.47153800959973", "module": "C2"}, {"value": "40.1967673994747", "module": "C3"}, {"value": "0", "module": "C4"}, {"value": "-1767.6383224683", "module": "D"}]}, "resolvedFlowVersion": "38.00.000", "flowProperties": [], "typeOfFlow": "Other flow", "classification": {"classHierarchy": "Quantities / Environmental quantities / EPD EN 15804 / LCI indicators", "name": "GaBiCategories"}}, {"dataSetInternalID": 4, "referenceToFlowDataSet": {"shortDescription": [{"value": "Nicht-erneuerbare Primärenergie als Energieträger (PENRE)", "lang": "de"}, {"value": "Non renewable primary energy as energy carrier (PENRE)", "lang": "en"}], "type": "flow data set", "refObjectId": "ac857178-2b45-46ec-892a-a9a4332f0372", "uri": "../flows/ac857178-2b45-46ec-892a-a9a4332f0372.xml"}, "exchange direction": "INPUT", "other": {"anies": [{"name": "referenceToUnitGroupDataSet", "value": {"shortDescription": [{"value": "MJ", "lang": "de"}], "type": "unit group data set", "refObjectId": "93a60a57-a3c8-11da-a746-0800200c9a66", "uri": "../unitgroups/93a60a57-a3c8-11da-a746-0800200c9a66.xml"}}, {"value": "5253.45022382618", "module": "A1-A3"}, {"value": "0", "module": "C1"}, {"value": "25.5520863872403", "module": "C2"}, {"value": "494.040206601561", "module": "C3"}, {"value": "0", "module": "C4"}, {"value": "-7020.94557589466", "module": "D"}]}, "resolvedFlowVersion": "38.00.000", "flowProperties": [], "typeOfFlow": "Other flow", "classification": {"classHierarchy": "Quantities", "name": "GaBiCategories"}}, {"dataSetInternalID": 5, "referenceToFlowDataSet": {"shortDescription": [{"value": "Nicht-erneuerbare Primärenergie zur stofflichen Nutzung (PENRM)", "lang": "de"}, {"value": "Non renewable primary energy as material utilization (PENRM)", "lang": "en"}], "type": "flow data set", "refObjectId": "1421caa0-679d-4bf4-b282-0eb850ccae27", "uri": "../flows/1421caa0-679d-4bf4-b282-0eb850ccae27.xml"}, "exchange direction": "INPUT", "other": {"anies": [{"name": "referenceToUnitGroupDataSet", "value": {"shortDescription": [{"value": "MJ", "lang": "de"}], "type": "unit group data set", "refObjectId": "93a60a57-a3c8-11da-a746-0800200c9a66", "uri": "../unitgroups/93a60a57-a3c8-11da-a746-0800200c9a66.xml"}}, {"value": "403.26747", "module": "A1-A3"}, {"value": "0", "module": "C1"}, {"value": "0", "module": "C2"}, {"value": "-403.26747", "module": "C3"}, {"value": "0", "module": "C4"}, {"value": "0", "module": "D"}]}, "resolvedFlowVersion": "38.00.000", "flowProperties": [], "typeOfFlow": "Other flow", "classification": {"classHierarchy": "Quantities", "name": "GaBiCategories"}}, {"dataSetInternalID": 6, "referenceToFlowDataSet": {"shortDescription": [{"value": "Total nicht erneuerbare Primärenergie (PENRT)", "lang": "de"}, {"value": "Total use of non renewable primary energy resources (PENRT)", "lang": "en"}], "type": "flow data set", "refObjectId": "06159210-646b-4c8d-8583-da9b3b95a6c1", "uri": "../flows/06159210-646b-4c8d-8583-da9b3b95a6c1.xml"}, "exchange direction": "INPUT", "other": {"anies": [{"name": "referenceToUnitGroupDataSet", "value": {"shortDescription": [{"value": "MJ", "lang": "de"}], "type": "unit group data set", "refObjectId": "93a60a57-a3c8-11da-a746-0800200c9a66", "uri": "../unitgroups/93a60a57-a3c8-11da-a746-0800200c9a66.xml"}}, {"value": "5656.71769382618", "module": "A1-A3"}, {"value": "0", "module": "C1"}, {"value": "25.5520863872403", "module": "C2"}, {"value": "90.7727366015608", "module": "C3"}, {"value": "0", "module": "C4"}, {"value": "-7020.94557589466", "module": "D"}]}, "resolvedFlowVersion": "38.00.000", "flowProperties": [], "typeOfFlow": "Other flow", "classification": {"classHierarchy": "Quantities / Environmental quantities / EPD EN 15804 / LCI indicators", "name": "GaBiCategories"}}, {"dataSetInternalID": 7, "referenceToFlowDataSet": {"shortDescription": [{"value": "Einsatz von Sekundärstoffen (SM)", "lang": "de"}, {"value": "Use of secondary material (SM)", "lang": "en"}], "type": "flow data set", "refObjectId": "c6a1f35f-2d09-4f54-8dfb-97e502e1ce92", "uri": "../flows/c6a1f35f-2d09-4f54-8dfb-97e502e1ce92.xml"}, "exchange direction": "INPUT", "other": {"anies": [{"name": "referenceToUnitGroupDataSet", "value": {"shortDescription": [{"value": "kg", "lang": "de"}], "type": "unit group data set", "refObjectId": "ad38d542-3fe9-439d-9b95-2f5f7752acaf", "uri": "../unitgroups/ad38d542-3fe9-439d-9b95-2f5f7752acaf.xml"}}, {"value": "0.25380888", "module": "A1-A3"}, {"value": "0", "module": "C1"}, {"value": "0", "module": "C2"}, {"value": "0", "module": "C3"}, {"value": "0", "module": "C4"}, {"value": "0", "module": "D"}]}, "resolvedFlowVersion": "38.00.000", "flowProperties": [], "typeOfFlow": "Other flow", "classification": {"classHierarchy": "Quantities / Environmental quantities / EPD EN 15804 / LCI indicators", "name": "GaBiCategories"}}, {"dataSetInternalID": 8, "referenceToFlowDataSet": {"shortDescription": [{"value": "Erneuerbare Sekundärbrennstoffe (RSF)", "lang": "de"}, {"value": "Use of renewable secondary fuels (RSF)", "lang": "en"}], "type": "flow data set", "refObjectId": "64333088-a55f-4aa2-9a31-c10b07816787", "uri": "../flows/64333088-a55f-4aa2-9a31-c10b07816787.xml"}, "exchange direction": "INPUT", "other": {"anies": [{"name": "referenceToUnitGroupDataSet", "value": {"shortDescription": [{"value": "MJ", "lang": "de"}], "type": "unit group data set", "refObjectId": "93a60a57-a3c8-11da-a746-0800200c9a66", "uri": "../unitgroups/93a60a57-a3c8-11da-a746-0800200c9a66.xml"}}, {"value": "3388.04376826815", "module": "A1-A3"}, {"value": "0", "module": "C1"}, {"value": "0", "module": "C2"}, {"value": "0", "module": "C3"}, {"value": "0", "module": "C4"}, {"value": "7695.02832349404", "module": "D"}]}, "resolvedFlowVersion": "38.00.000", "flowProperties": [], "typeOfFlow": "Other flow", "classification": {"classHierarchy": "Quantities / Environmental quantities / EPD EN 15804 / LCI indicators", "name": "GaBiCategories"}}, {"dataSetInternalID": 9, "referenceToFlowDataSet": {"shortDescription": [{"value": "Nicht erneuerbare Sekundärbrennstoffe (NRSF)", "lang": "de"}, {"value": "Use of non renewable secondary fuels (NRSF)", "lang": "en"}], "type": "flow data set", "refObjectId": "89def144-d39a-4287-b86f-efde453ddcb2", "uri": "../flows/89def144-d39a-4287-b86f-efde453ddcb2.xml"}, "exchange direction": "INPUT", "other": {"anies": [{"name": "referenceToUnitGroupDataSet", "value": {"shortDescription": [{"value": "MJ", "lang": "de"}], "type": "unit group data set", "refObjectId": "93a60a57-a3c8-11da-a746-0800200c9a66", "uri": "../unitgroups/93a60a57-a3c8-11da-a746-0800200c9a66.xml"}}, {"value": "0", "module": "A1-A3"}, {"value": "0", "module": "C1"}, {"value": "0", "module": "C2"}, {"value": "0", "module": "C3"}, {"value": "0", "module": "C4"}, {"value": "307.532428341463", "module": "D"}]}, "resolvedFlowVersion": "38.00.000", "flowProperties": [], "typeOfFlow": "Other flow", "classification": {"classHierarchy": "Quantities / Environmental quantities / EPD EN 15804 / LCI indicators", "name": "GaBiCategories"}}, {"dataSetInternalID": 10, "referenceToFlowDataSet": {"shortDescription": [{"value": "Einsatz von Süßwasserressourcen (FW)", "lang": "de"}, {"value": "Use of net fresh water (FW)", "lang": "en"}], "type": "flow data set", "refObjectId": "3cf952c8-f3a4-461d-8c96-96456ca62246", "uri": "../flows/3cf952c8-f3a4-461d-8c96-96456ca62246.xml"}, "exchange direction": "INPUT", "other": {"anies": [{"name": "referenceToUnitGroupDataSet", "value": {"shortDescription": [{"value": "m^3", "lang": "de"}], "type": "unit group data set", "refObjectId": "cd950537-0a98-4044-9ba7-9f9a68d0a504", "uri": "../unitgroups/cd950537-0a98-4044-9ba7-9f9a68d0a504.xml"}}, {"value": "1.17181477487247", "module": "A1-A3"}, {"value": "0", "module": "C1"}, {"value": "0.00171483726227553", "module": "C2"}, {"value": "0.0464778348341248", "module": "C3"}, {"value": "0", "module": "C4"}, {"value": "-1.42958705664455", "module": "D"}]}, "resolvedFlowVersion": "38.00.000", "flowProperties": [], "typeOfFlow": "Other flow", "classification": {"classHierarchy": "Quantities / Environmental quantities / EPD EN 15804 / LCI indicators", "name": "GaBiCategories"}}, {"dataSetInternalID": 11, "referenceToFlowDataSet": {"shortDescription": [{"value": "Gefährlicher Abfall zur Deponie (HWD)", "lang": "de"}, {"value": "Hazardous waste disposed (HWD)", "lang": "en"}], "type": "flow data set", "refObjectId": "430f9e0f-59b2-46a0-8e0d-55e0e84948fc", "uri": "../flows/430f9e0f-59b2-46a0-8e0d-55e0e84948fc.xml"}, "exchange direction": "OUTPUT", "other": {"anies": [{"name": "referenceToUnitGroupDataSet", "value": {"shortDescription": [{"value": "kg", "lang": "de"}], "type": "unit group data set", "refObjectId": "ad38d542-3fe9-439d-9b95-2f5f7752acaf", "uri": "../unitgroups/ad38d542-3fe9-439d-9b95-2f5f7752acaf.xml"}}, {"value": "1.7890271255182E-05", "module": "A1-A3"}, {"value": "0", "module": "C1"}, {"value": "1.18157004393063E-06", "module": "C2"}, {"value": "3.75518565819245E-08", "module": "C3"}, {"value": "0", "module": "C4"}, {"value": "-2.37613831871282E-06", "module": "D"}]}, "resolvedFlowVersion": "38.00.000", "flowProperties": [], "typeOfFlow": "Other flow", "classification": {"classHierarchy": "Quantities / Environmental quantities / EPD EN 15804 / LCI indicators", "name": "GaBiCategories"}}, {"dataSetInternalID": 12, "referenceToFlowDataSet": {"shortDescription": [{"value": "Entsorgter nicht gefährlicher Abfall (NHWD)", "lang": "de"}, {"value": "Non hazardous waste disposed (NHWD)", "lang": "en"}], "type": "flow data set", "refObjectId": "b29ef66b-e286-4afa-949f-62f1a7b4d7fa", "uri": "../flows/b29ef66b-e286-4afa-949f-62f1a7b4d7fa.xml"}, "exchange direction": "OUTPUT", "other": {"anies": [{"name": "referenceToUnitGroupDataSet", "value": {"shortDescription": [{"value": "kg", "lang": "de"}], "type": "unit group data set", "refObjectId": "ad38d542-3fe9-439d-9b95-2f5f7752acaf", "uri": "../unitgroups/ad38d542-3fe9-439d-9b95-2f5f7752acaf.xml"}}, {"value": "10.0513724954127", "module": "A1-A3"}, {"value": "0", "module": "C1"}, {"value": "0.00404980827723245", "module": "C2"}, {"value": "0.064355788727499", "module": "C3"}, {"value": "0", "module": "C4"}, {"value": "0.256677904614124", "module": "D"}]}, "resolvedFlowVersion": "38.00.000", "flowProperties": [], "typeOfFlow": "Other flow", "classification": {"classHierarchy": "Quantities / Environmental quantities / EPD EN 15804 / LCI indicators", "name": "GaBiCategories"}}, {"dataSetInternalID": 13, "referenceToFlowDataSet": {"shortDescription": [{"value": "Entsorgter radioaktiver Abfall (RWD)", "lang": "de"}, {"value": "Radioactive waste disposed (RWD)", "lang": "en"}], "type": "flow data set", "refObjectId": "3449546e-52ad-4b39-b809-9fb77cea8ff6", "uri": "../flows/3449546e-52ad-4b39-b809-9fb77cea8ff6.xml"}, "exchange direction": "OUTPUT", "other": {"anies": [{"name": "referenceToUnitGroupDataSet", "value": {"shortDescription": [{"value": "kg", "lang": "de"}], "type": "unit group data set", "refObjectId": "ad38d542-3fe9-439d-9b95-2f5f7752acaf", "uri": "../unitgroups/ad38d542-3fe9-439d-9b95-2f5f7752acaf.xml"}}, {"value": "0.160543885620331", "module": "A1-A3"}, {"value": "0", "module": "C1"}, {"value": "4.70949237398518E-05", "module": "C2"}, {"value": "0.0137636225856841", "module": "C3"}, {"value": "0", "module": "C4"}, {"value": "-0.604347283349534", "module": "D"}]}, "resolvedFlowVersion": "38.00.000", "flowProperties": [], "typeOfFlow": "Other flow", "classification": {"classHierarchy": "Quantities / Environmental quantities / EPD EN 15804 / LCI indicators", "name": "GaBiCategories"}}, {"dataSetInternalID": 14, "referenceToFlowDataSet": {"shortDescription": [{"value": "Komponenten für die Wiederverwendung (CRU)", "lang": "de"}, {"value": "Components for re-use (CRU)", "lang": "en"}], "type": "flow data set", "refObjectId": "a2b32f97-3fc7-4af2-b209-525bc6426f33", "uri": "../flows/a2b32f97-3fc7-4af2-b209-525bc6426f33.xml"}, "exchange direction": "OUTPUT", "other": {"anies": [{"name": "referenceToUnitGroupDataSet", "value": {"shortDescription": [{"value": "kg", "lang": "de"}], "type": "unit group data set", "refObjectId": "ad38d542-3fe9-439d-9b95-2f5f7752acaf", "uri": "../unitgroups/ad38d542-3fe9-439d-9b95-2f5f7752acaf.xml"}}, {"value": "0", "module": "A1-A3"}, {"value": "0", "module": "C1"}, {"value": "0", "module": "C2"}, {"value": "0", "module": "C3"}, {"value": "0", "module": "C4"}, {"value": "0", "module": "D"}]}, "resolvedFlowVersion": "38.00.000", "flowProperties": [], "typeOfFlow": "Other flow", "classification": {"classHierarchy": "Quantities / Environmental quantities / EPD EN 15804 / LCI indicators", "name": "GaBiCategories"}}, {"dataSetInternalID": 15, "referenceToFlowDataSet": {"shortDescription": [{"value": "Stoffe zum Recycling (MFR)", "lang": "de"}, {"value": "Materials for recycling (MFR)", "lang": "en"}], "type": "flow data set", "refObjectId": "d7fe48a5-4103-49c8-9aae-b0b5dfdbd6ae", "uri": "../flows/d7fe48a5-4103-49c8-9aae-b0b5dfdbd6ae.xml"}, "exchange direction": "OUTPUT", "other": {"anies": [{"name": "referenceToUnitGroupDataSet", "value": {"shortDescription": [{"value": "kg", "lang": "de"}], "type": "unit group data set", "refObjectId": "ad38d542-3fe9-439d-9b95-2f5f7752acaf", "uri": "../unitgroups/ad38d542-3fe9-439d-9b95-2f5f7752acaf.xml"}}, {"value": "0", "module": "A1-A3"}, {"value": "0", "module": "C1"}, {"value": "0", "module": "C2"}, {"value": "0", "module": "C3"}, {"value": "0", "module": "C4"}, {"value": "0", "module": "D"}]}, "resolvedFlowVersion": "38.00.000", "flowProperties": [], "typeOfFlow": "Other flow", "classification": {"classHierarchy": "Quantities / Environmental quantities / EPD EN 15804 / LCI indicators", "name": "GaBiCategories"}}, {"dataSetInternalID": 16, "referenceToFlowDataSet": {"shortDescription": [{"value": "Stoffe für die Energierückgewinnung (MER)", "lang": "de"}, {"value": "Materials for energy recovery (MER)", "lang": "en"}], "type": "flow data set", "refObjectId": "59a9181c-3aaf-46ee-8b13-2b3723b6e447", "uri": "../flows/59a9181c-3aaf-46ee-8b13-2b3723b6e447.xml"}, "exchange direction": "OUTPUT", "other": {"anies": [{"name": "referenceToUnitGroupDataSet", "value": {"shortDescription": [{"value": "kg", "lang": "de"}], "type": "unit group data set", "refObjectId": "ad38d542-3fe9-439d-9b95-2f5f7752acaf", "uri": "../unitgroups/ad38d542-3fe9-439d-9b95-2f5f7752acaf.xml"}}, {"value": "0", "module": "A1-A3"}, {"value": "0", "module": "C1"}, {"value": "0", "module": "C2"}, {"value": "640.744186046512", "module": "C3"}, {"value": "0", "module": "C4"}, {"value": "0", "module": "D"}]}, "resolvedFlowVersion": "38.00.000", "flowProperties": [], "typeOfFlow": "Other flow", "classification": {"classHierarchy": "Quantities / Environmental quantities / EPD EN 15804 / LCI indicators", "name": "GaBiCategories"}}, {"dataSetInternalID": 17, "referenceToFlowDataSet": {"shortDescription": [{"value": "Exportierte elektrische Energie (EEE)", "lang": "de"}, {"value": "Exported electrical energy (EEE)", "lang": "en"}], "type": "flow data set", "refObjectId": "4da0c987-2b76-40d6-9e9e-82a017aaaf29", "uri": "../flows/4da0c987-2b76-40d6-9e9e-82a017aaaf29.xml"}, "exchange direction": "OUTPUT", "other": {"anies": [{"name": "referenceToUnitGroupDataSet", "value": {"shortDescription": [{"value": "MJ", "lang": "de"}], "type": "unit group data set", "refObjectId": "93a60a57-a3c8-11da-a746-0800200c9a66", "uri": "../unitgroups/93a60a57-a3c8-11da-a746-0800200c9a66.xml"}}, {"value": "0", "module": "A1-A3"}, {"value": "0", "module": "C1"}, {"value": "0", "module": "C2"}, {"value": "0", "module": "C3"}, {"value": "0", "module": "C4"}, {"value": "0", "module": "D"}]}, "resolvedFlowVersion": "38.00.000", "flowProperties": [], "typeOfFlow": "Other flow", "classification": {"classHierarchy": "Quantities / Environmental quantities / EPD EN 15804 / LCI indicators", "name": "GaBiCategories"}}, {"dataSetInternalID": 18, "referenceToFlowDataSet": {"shortDescription": [{"value": "Exportierte thermische Energie (EET)", "lang": "de"}, {"value": "Exported thermal energy (EET)", "lang": "en"}], "type": "flow data set", "refObjectId": "98daf38a-7a79-46d3-9a37-2b7bd0955810", "uri": "../flows/98daf38a-7a79-46d3-9a37-2b7bd0955810.xml"}, "exchange direction": "OUTPUT", "other": {"anies": [{"name": "referenceToUnitGroupDataSet", "value": {"shortDescription": [{"value": "MJ", "lang": "de"}], "type": "unit group data set", "refObjectId": "93a60a57-a3c8-11da-a746-0800200c9a66", "uri": "../unitgroups/93a60a57-a3c8-11da-a746-0800200c9a66.xml"}}, {"value": "0", "module": "A1-A3"}, {"value": "0", "module": "C1"}, {"value": "0", "module": "C2"}, {"value": "0", "module": "C3"}, {"value": "0", "module": "C4"}, {"value": "0", "module": "D"}]}, "resolvedFlowVersion": "38.00.000", "flowProperties": [], "typeOfFlow": "Other flow", "classification": {"classHierarchy": "Quantities / Environmental quantities / EPD EN 15804 / LCI indicators", "name": "GaBiCategories"}}]}, "LCIAResults": {"LCIAResult": [{"referenceToLCIAMethodDataSet": {"shortDescription": [{"value": "Globales Erwärmungspotenzial total (GWP-total)", "lang": "de"}, {"value": "Global Warming Potential total (GWP-total)", "lang": "en"}], "type": "LCIA method data set", "refObjectId": "6a37f984-a4b3-458a-a20a-64418c145fa2", "uri": "../lciamethods/6a37f984-a4b3-458a-a20a-64418c145fa2.xml"}, "other": {"anies": [{"name": "referenceToUnitGroupDataSet", "value": {"shortDescription": [{"value": "kg CO_(2)-Äq.", "lang": "de"}], "type": "unit group data set", "refObjectId": "1ebf3012-d0db-4de2-aefd-ef30cedb0be1", "uri": "../unitgroups/1ebf3012-d0db-4de2-aefd-ef30cedb0be1.xml"}}, {"value": "-583.691306059584", "module": "A1-A3"}, {"value": "0", "module": "C1"}, {"value": "1.93069369361257", "module": "C2"}, {"value": "998.33830184975", "module": "C3"}, {"value": "0", "module": "C4"}, {"value": "-351.892738489744", "module": "D"}]}}, {"referenceToLCIAMethodDataSet": {"shortDescription": [{"value": "Globales Erwärmungspotenzial fossil (GWP-fossil)", "lang": "de"}, {"value": "Global Warming Potential fossil fuels (GWP-fossil)", "lang": "en"}], "type": "LCIA method data set", "refObjectId": "5f635281-343e-44fb-83df-1971b155e6b6", "uri": "../lciamethods/5f635281-343e-44fb-83df-1971b155e6b6.xml"}, "other": {"anies": [{"name": "referenceToUnitGroupDataSet", "value": {"shortDescription": [{"value": "kg CO_(2)-Äq.", "lang": "de"}], "type": "unit group data set", "refObjectId": "1ebf3012-d0db-4de2-aefd-ef30cedb0be1", "uri": "../unitgroups/1ebf3012-d0db-4de2-aefd-ef30cedb0be1.xml"}}, {"value": "398.328028558228", "module": "A1-A3"}, {"value": "0", "module": "C1"}, {"value": "1.91845598358514", "module": "C2"}, {"value": "5.16013365666023", "module": "C3"}, {"value": "0", "module": "C4"}, {"value": "-350.536793223314", "module": "D"}]}}, {"referenceToLCIAMethodDataSet": {"shortDescription": [{"value": "Globales Erwärmungspotenzial biogen (GWP-biogenic)", "lang": "de"}, {"value": "Global Warming Potential biogenic (GWP-biogenic)", "lang": "en"}], "type": "LCIA method data set", "refObjectId": "2356e1ab-0185-4db5-86e5-16de51c7485c", "uri": "../lciamethods/2356e1ab-0185-4db5-86e5-16de51c7485c.xml"}, "other": {"anies": [{"name": "referenceToUnitGroupDataSet", "value": {"shortDescription": [{"value": "kg CO_(2)-Äq.", "lang": "de"}], "type": "unit group data set", "refObjectId": "1ebf3012-d0db-4de2-aefd-ef30cedb0be1", "uri": "../unitgroups/1ebf3012-d0db-4de2-aefd-ef30cedb0be1.xml"}}, {"value": "-982.562764478588", "module": "A1-A3"}, {"value": "0", "module": "C1"}, {"value": "-0.00320217923528393", "module": "C2"}, {"value": "993.170692035142", "module": "C3"}, {"value": "0", "module": "C4"}, {"value": "-1.02406399946537", "module": "D"}]}}, {"referenceToLCIAMethodDataSet": {"shortDescription": [{"value": "Globales Erwärmungspotenzial luluc (GWP-luluc)", "lang": "de"}, {"value": "Global Warming Potential luluc (GWP-luluc)", "lang": "en"}], "type": "LCIA method data set", "refObjectId": "4331bbdb-978a-490d-8707-eeb047f01a55", "uri": "../lciamethods/4331bbdb-978a-490d-8707-eeb047f01a55.xml"}, "other": {"anies": [{"name": "referenceToUnitGroupDataSet", "value": {"shortDescription": [{"value": "kg CO_(2)-Äq.", "lang": "de"}], "type": "unit group data set", "refObjectId": "1ebf3012-d0db-4de2-aefd-ef30cedb0be1", "uri": "../unitgroups/1ebf3012-d0db-4de2-aefd-ef30cedb0be1.xml"}}, {"value": "0.54342986077593", "module": "A1-A3"}, {"value": "0", "module": "C1"}, {"value": "0.0154398892627093", "module": "C2"}, {"value": "0.0074761579481156", "module": "C3"}, {"value": "0", "module": "C4"}, {"value": "-0.331881266964981", "module": "D"}]}}, {"referenceToLCIAMethodDataSet": {"shortDescription": [{"value": "Abbau Potential der stratosphärischen Ozonschicht (ODP)", "lang": "de"}, {"value": "Depletion potential of the stratospheric ozone layer (ODP)", "lang": "en"}], "type": "LCIA method data set", "refObjectId": "b5c629d6-def3-11e6-bf01-fe55135034f3", "uri": "../lciamethods/b5c629d6-def3-11e6-bf01-fe55135034f3.xml"}, "other": {"anies": [{"name": "referenceToUnitGroupDataSet", "value": {"shortDescription": [{"value": "kg CFC11-Äq.", "lang": "de"}], "type": "unit group data set", "refObjectId": "d9e957c9-7309-4474-bf3a-7777df6c4e5b", "uri": "../unitgroups/d9e957c9-7309-4474-bf3a-7777df6c4e5b.xml"}}, {"value": "1.60130167409258E-11", "module": "A1-A3"}, {"value": "0", "module": "C1"}, {"value": "3.50086090909945E-16", "module": "C2"}, {"value": "1.13478739968269E-13", "module": "C3"}, {"value": "0", "module": "C4"}, {"value": "-4.97884220597024E-12", "module": "D"}]}}, {"referenceToLCIAMethodDataSet": {"shortDescription": [{"value": "Versauerungspotenzial von Boden und Wasser (AP)", "lang": "de"}, {"value": "Acidification potential of land and water (AP)", "lang": "en"}], "type": "LCIA method data set", "refObjectId": "b5c611c6-def3-11e6-bf01-fe55135034f3", "uri": "../lciamethods/b5c611c6-def3-11e6-bf01-fe55135034f3.xml"}, "other": {"anies": [{"name": "referenceToUnitGroupDataSet", "value": {"shortDescription": [{"value": "mol H^(+)-Äq.", "lang": "de"}], "type": "unit group data set", "refObjectId": "42e089ac-92bf-4bf2-8ca1-5fc40d18f2ed", "uri": "../unitgroups/42e089ac-92bf-4bf2-8ca1-5fc40d18f2ed.xml"}}, {"value": "0.873188001214901", "module": "A1-A3"}, {"value": "0", "module": "C1"}, {"value": "0.00648290676077547", "module": "C2"}, {"value": "0.0113928414238562", "module": "C3"}, {"value": "0", "module": "C4"}, {"value": "0.273432436894614", "module": "D"}]}}, {"referenceToLCIAMethodDataSet": {"shortDescription": [{"value": "Eutrophierungspotenzial Süßwasser (EP-freshwater)", "lang": "de"}, {"value": "Eutrophication potential aquatic freshwater (EP-freshwater)", "lang": "en"}], "type": "LCIA method data set", "refObjectId": "b53ec18f-7377-4ad3-86eb-cc3f4f276b2b", "uri": "../lciamethods/b53ec18f-7377-4ad3-86eb-cc3f4f276b2b.xml"}, "other": {"anies": [{"name": "referenceToUnitGroupDataSet", "value": {"shortDescription": [{"value": "kg P-Äq.", "lang": "de"}], "type": "unit group data set", "refObjectId": "0429039d-a61d-4590-ba67-aa4a20a810a1", "uri": "../unitgroups/0429039d-a61d-4590-ba67-aa4a20a810a1.xml"}}, {"value": "0.00115696176514231", "module": "A1-A3"}, {"value": "0", "module": "C1"}, {"value": "5.80994961010429E-06", "module": "C2"}, {"value": "1.37827359350005E-05", "module": "C3"}, {"value": "0", "module": "C4"}, {"value": "-0.000609803524660532", "module": "D"}]}}, {"referenceToLCIAMethodDataSet": {"shortDescription": [{"value": "Eutrophierungspotenzial Salzwasser (EP-marine)", "lang": "de"}, {"value": "Eutrophication potential aquatic marine (EP-marine)", "lang": "en"}], "type": "LCIA method data set", "refObjectId": "b5c619fa-def3-11e6-bf01-fe55135034f3", "uri": "../lciamethods/b5c619fa-def3-11e6-bf01-fe55135034f3.xml"}, "other": {"anies": [{"name": "referenceToUnitGroupDataSet", "value": {"shortDescription": [{"value": "kg N-Äq.", "lang": "de"}], "type": "unit group data set", "refObjectId": "d05bb823-ecdf-4686-8c40-bf1d9257859f", "uri": "../unitgroups/d05bb823-ecdf-4686-8c40-bf1d9257859f.xml"}}, {"value": "0.342499172506243", "module": "A1-A3"}, {"value": "0", "module": "C1"}, {"value": "0.00292466271911234", "module": "C2"}, {"value": "0.00253031154220984", "module": "C3"}, {"value": "0", "module": "C4"}, {"value": "0.0693454132467154", "module": "D"}]}}, {"referenceToLCIAMethodDataSet": {"shortDescription": [{"value": "Eutrophierungspotenzial Land (EP-terrestrial)", "lang": "de"}, {"value": "Eutrophication potential terrestrial (EP-terrestrial)", "lang": "en"}], "type": "LCIA method data set", "refObjectId": "b5c614d2-def3-11e6-bf01-fe55135034f3", "uri": "../lciamethods/b5c614d2-def3-11e6-bf01-fe55135034f3.xml"}, "other": {"anies": [{"name": "referenceToUnitGroupDataSet", "value": {"shortDescription": [{"value": "mol N-Äq.", "lang": "de"}], "type": "unit group data set", "refObjectId": "71b4d617-0ec9-4d3f-b65e-e438940c2401", "uri": "../unitgroups/71b4d617-0ec9-4d3f-b65e-e438940c2401.xml"}}, {"value": "3.68729180738638", "module": "A1-A3"}, {"value": "0", "module": "C1"}, {"value": "0.0326702907782105", "module": "C2"}, {"value": "0.026584062528189", "module": "C3"}, {"value": "0", "module": "C4"}, {"value": "0.824153522961292", "module": "D"}]}}, {"referenceToLCIAMethodDataSet": {"shortDescription": [{"value": "Bildungspotential für troposphärisches Ozon (POCP)", "lang": "de"}, {"value": "Formation potential of tropospheric ozone photochemical oxidants (POCP)", "lang": "en"}], "type": "LCIA method data set", "refObjectId": "b5c610fe-def3-11e6-bf01-fe55135034f3", "uri": "../lciamethods/b5c610fe-def3-11e6-bf01-fe55135034f3.xml"}, "other": {"anies": [{"name": "referenceToUnitGroupDataSet", "value": {"shortDescription": [{"value": "kg NMVOC-Äq.", "lang": "de"}], "type": "unit group data set", "refObjectId": "d27c25f8-fbc1-44c6-b47b-4adbae4199c6", "uri": "../unitgroups/d27c25f8-fbc1-44c6-b47b-4adbae4199c6.xml"}}, {"value": "0.988203111471163", "module": "A1-A3"}, {"value": "0", "module": "C1"}, {"value": "0.00574604486565877", "module": "C2"}, {"value": "0.00693432029289997", "module": "C3"}, {"value": "0", "module": "C4"}, {"value": "0.29290058474446", "module": "D"}]}}, {"referenceToLCIAMethodDataSet": {"shortDescription": [{"value": "Potenzial für den abiotischen Abbau nicht fossiler Ressourcen (ADPE)", "lang": "de"}, {"value": "Abiotic depletion potential for non fossil resources (ADPE)", "lang": "en"}], "type": "LCIA method data set", "refObjectId": "b2ad6494-c78d-11e6-9d9d-cec0c932ce01", "uri": "../lciamethods/b2ad6494-c78d-11e6-9d9d-cec0c932ce01.xml"}, "other": {"anies": [{"name": "referenceToUnitGroupDataSet", "value": {"shortDescription": [{"value": "kg Sb-Äq.", "lang": "de"}], "type": "unit group data set", "refObjectId": "54ccd2d9-a32a-4fc2-923d-f2c8c93e89d4", "uri": "../unitgroups/54ccd2d9-a32a-4fc2-923d-f2c8c93e89d4.xml"}}, {"value": "0.000270614461334983", "module": "A1-A3"}, {"value": "0", "module": "C1"}, {"value": "1.5424183860292E-07", "module": "C2"}, {"value": "1.49330054987502E-06", "module": "C3"}, {"value": "0", "module": "C4"}, {"value": "-7.48580218360416E-05", "module": "D"}]}}, {"referenceToLCIAMethodDataSet": {"shortDescription": [{"value": "Potenzial für den abiotischen Abbau fossiler Brennstoffe (ADPF)", "lang": "de"}, {"value": "Abiotic depletion potential for fossil resources (ADPF)", "lang": "en"}], "type": "LCIA method data set", "refObjectId": "b2ad6110-c78d-11e6-9d9d-cec0c932ce01", "uri": "../lciamethods/b2ad6110-c78d-11e6-9d9d-cec0c932ce01.xml"}, "other": {"anies": [{"name": "referenceToUnitGroupDataSet", "value": {"shortDescription": [{"value": "MJ", "lang": "de"}], "type": "unit group data set", "refObjectId": "93a60a57-a3c8-11da-a746-0800200c9a66", "uri": "../unitgroups/93a60a57-a3c8-11da-a746-0800200c9a66.xml"}}, {"value": "5655.27009089583", "module": "A1-A3"}, {"value": "0", "module": "C1"}, {"value": "25.4500503294086", "module": "C2"}, {"value": "90.75434401395", "module": "C3"}, {"value": "0", "module": "C4"}, {"value": "-7020.1181478313", "module": "D"}]}}, {"referenceToLCIAMethodDataSet": {"shortDescription": [{"value": "Wassernutzung (WDP)", "lang": "de"}, {"value": "Water use (WDP)", "lang": "en"}], "type": "LCIA method data set", "refObjectId": "b2ad66ce-c78d-11e6-9d9d-cec0c932ce01", "uri": "../lciamethods/b2ad66ce-c78d-11e6-9d9d-cec0c932ce01.xml"}, "other": {"anies": [{"name": "referenceToUnitGroupDataSet", "value": {"shortDescription": [{"value": "m^(3) Welt-Äq. entzogen", "lang": "de"}], "type": "unit group data set", "refObjectId": "6ae2df01-888e-46c8-b17d-49fa3869b476", "uri": "../unitgroups/6ae2df01-888e-46c8-b17d-49fa3869b476.xml"}}, {"value": "2.78567533891282", "module": "A1-A3"}, {"value": "0", "module": "C1"}, {"value": "0.01859987520474", "module": "C2"}, {"value": "1.12444799421465", "module": "C3"}, {"value": "0", "module": "C4"}, {"value": "-22.9757358005791", "module": "D"}]}}, {"referenceToLCIAMethodDataSet": {"shortDescription": [{"value": "Auftreten von Krankheiten aufgrund von Feinstaubemissionen (PM)", "lang": "de"}, {"value": "Incidence of disease due to PM emissions (PM)", "lang": "en"}], "type": "LCIA method data set", "refObjectId": "b5c602c6-def3-11e6-bf01-fe55135034f3", "uri": "../lciamethods/b5c602c6-def3-11e6-bf01-fe55135034f3.xml"}, "other": {"anies": [{"name": "referenceToUnitGroupDataSet", "value": {"shortDescription": [{"value": "Krankheitsfälle", "lang": "de"}], "type": "unit group data set", "refObjectId": "3883559b-648f-4afc-8ba2-0bd24f3affa3", "uri": "../unitgroups/3883559b-648f-4afc-8ba2-0bd24f3affa3.xml"}}, {"value": "0.00200452286613798", "module": "A1-A3"}, {"value": "0", "module": "C1"}, {"value": "3.66301739755352E-08", "module": "C2"}, {"value": "9.55522894310366E-08", "module": "C3"}, {"value": "0", "module": "C4"}, {"value": "-1.47889142134604E-06", "module": "D"}]}}, {"referenceToLCIAMethodDataSet": {"shortDescription": [{"value": "Wirkung durch Exposition des Menschen mit U235 (IR)", "lang": "de"}, {"value": "Human exposure efficiency relative to U235 (IR)", "lang": "en"}], "type": "LCIA method data set", "refObjectId": "b5c632be-def3-11e6-bf01-fe55135034f3", "uri": "../lciamethods/b5c632be-def3-11e6-bf01-fe55135034f3.xml"}, "other": {"anies": [{"name": "referenceToUnitGroupDataSet", "value": {"shortDescription": [{"value": "kBq U235-Äq.", "lang": "de"}], "type": "unit group data set", "refObjectId": "456b05bf-1415-44a9-9993-02452f554c09", "uri": "../unitgroups/456b05bf-1415-44a9-9993-02452f554c09.xml"}}, {"value": "14.5677814604939", "module": "A1-A3"}, {"value": "0", "module": "C1"}, {"value": "0.00694767068089727", "module": "C2"}, {"value": "2.25814425284603", "module": "C3"}, {"value": "0", "module": "C4"}, {"value": "-99.148740606846", "module": "D"}]}}, {"referenceToLCIAMethodDataSet": {"shortDescription": [{"value": "Toxizitätsvergleichseinheit für Ökosysteme (ETP-fw)", "lang": "de"}, {"value": "Comparative toxic unit for ecosystems (ETP-fw)", "lang": "en"}], "type": "LCIA method data set", "refObjectId": "ee1082d1-b0f7-43ca-a1f0-21e2a4a74511", "uri": "../lciamethods/ee1082d1-b0f7-43ca-a1f0-21e2a4a74511.xml"}, "other": {"anies": [{"name": "referenceToUnitGroupDataSet", "value": {"shortDescription": [{"value": "CTUe", "lang": "de"}], "type": "unit group data set", "refObjectId": "aa959ded-f1eb-4efb-9c5c-2d60be36b3e6", "uri": "../unitgroups/aa959ded-f1eb-4efb-9c5c-2d60be36b3e6.xml"}}, {"value": "2904.20591780679", "module": "A1-A3"}, {"value": "0", "module": "C1"}, {"value": "19.0415705910462", "module": "C2"}, {"value": "38.8397514404267", "module": "C3"}, {"value": "0", "module": "C4"}, {"value": "-1719.44718239933", "module": "D"}]}}, {"referenceToLCIAMethodDataSet": {"shortDescription": [{"value": "Toxizitätsvergleichseinheit für Menschen (krebserregend) (HTP-c)", "lang": "de"}, {"value": "Comparative toxic unit for humans (carcinogenic) (HTP-c)", "lang": "en"}], "type": "LCIA method data set", "refObjectId": "2299222a-bbd8-474f-9d4f-4dd1f18aea7c", "uri": "../lciamethods/2299222a-bbd8-474f-9d4f-4dd1f18aea7c.xml"}, "other": {"anies": [{"name": "referenceToUnitGroupDataSet", "value": {"shortDescription": [{"value": "CTUh", "lang": "de"}], "type": "unit group data set", "refObjectId": "d4c9523e-2d7e-49fd-8469-998f547d3a70", "uri": "../unitgroups/d4c9523e-2d7e-49fd-8469-998f547d3a70.xml"}}, {"value": "4.48308189501918E-07", "module": "A1-A3"}, {"value": "0", "module": "C1"}, {"value": "3.93562920964799E-10", "module": "C2"}, {"value": "1.07250893232372E-09", "module": "C3"}, {"value": "0", "module": "C4"}, {"value": "-6.80029022653621E-09", "module": "D"}]}}, {"referenceToLCIAMethodDataSet": {"shortDescription": [{"value": "Toxizitätsvergleichseinheit für Menschen (nicht krebserregend) (HTP-nc)", "lang": "de"}, {"value": "Comparative toxic unit for humans (noncarcinogenic) (HTP-nc)", "lang": "en"}], "type": "LCIA method data set", "refObjectId": "3af763a5-b7a1-48c9-9cee-1f223481fcef", "uri": "../lciamethods/3af763a5-b7a1-48c9-9cee-1f223481fcef.xml"}, "other": {"anies": [{"name": "referenceToUnitGroupDataSet", "value": {"shortDescription": [{"value": "CTUh", "lang": "de"}], "type": "unit group data set", "refObjectId": "d4c9523e-2d7e-49fd-8469-998f547d3a70", "uri": "../unitgroups/d4c9523e-2d7e-49fd-8469-998f547d3a70.xml"}}, {"value": "3.81575239177602E-06", "module": "A1-A3"}, {"value": "0", "module": "C1"}, {"value": "2.26772622490746E-08", "module": "C2"}, {"value": "3.95155839425602E-08", "module": "C3"}, {"value": "0", "module": "C4"}, {"value": "1.98759106512134E-06", "module": "D"}]}}, {"referenceToLCIAMethodDataSet": {"shortDescription": [{"value": "Bodenqualitätsindex (SQP)", "lang": "de"}, {"value": "Soil quality index (SQP)", "lang": "en"}], "type": "LCIA method data set", "refObjectId": "b2ad6890-c78d-11e6-9d9d-cec0c932ce01", "uri": "../lciamethods/b2ad6890-c78d-11e6-9d9d-cec0c932ce01.xml"}, "other": {"anies": [{"name": "referenceToUnitGroupDataSet", "value": {"shortDescription": [{"value": "SQP", "lang": "de"}], "type": "unit group data set", "refObjectId": "f130951c-e67f-4f7f-8dd4-665de3974e18", "uri": "../unitgroups/f130951c-e67f-4f7f-8dd4-665de3974e18.xml"}}, {"value": "80368.3957382862", "module": "A1-A3"}, {"value": "0", "module": "C1"}, {"value": "8.93325763947682", "module": "C2"}, {"value": "28.8838875188267", "module": "C3"}, {"value": "0", "module": "C4"}, {"value": "-1291.06722081511", "module": "D"}]}}]}, "otherAttributes": {"{http://www.indata.network/EPD/2019}epd-version": "1.2"}, "version": "1.1", "locations": "../ILCDLocations.xml"}