{"processInformation": {"dataSetInformation": {"UUID": "5a90eb60-dce3-4a0b-bfd5-b55eabaa6bb9", "name": {"baseName": [{"value": "Warmumgeformte Stahlpressteile (\"phs-ultraform\")", "lang": "de"}, {"value": "Hot-formed press-hardened steel components (\"phs-ultraform\")", "lang": "en"}], "functionalUnitFlowProperties": [{"lang": "de"}]}, "classificationInformation": {"classification": [{"class": [{"value": "Metalle", "level": 0, "classId": "4"}, {"value": "Stahl und Eisen", "level": 1, "classId": "4.1"}, {"value": "Stahlbleche", "level": 2, "classId": "4.1.04"}], "name": "OEKOBAU.DAT"}, {"class": [{"value": "02 Bauprodukte", "level": 0}, {"value": "Metallbauprodukte und Zubehör", "level": 1}, {"value": "Dünnwandige Profile und Profiltafeln aus Metall", "level": 2}], "name": "IBUCategories"}]}, "generalComment": [{"value": "phs-Bauteile (= press hardened steel, pressgehärtete Stähle) umfassen eine Produktgruppe, die sich durch äußerst hohe Festigkeit am Fertigbauteil bei sehr guten Umformmöglichkeiten in der Produktherstellung auszeichnen. In der vorliegenden Durchschnittsbetrachtung werden verschiedene Verarbeitungsvarianten von unterschiedlichen Herstellungsstandorten der voestalpine Metal Forming Division zusammengefasst.\n\n„phs-ultraform“ ist eine registrierte Marke der voestalpine Stahl GmbH.\n\nphs-ultraform (EUIPO Registrierungsnummern 013290044 und 005772165): Kaltumgeformte Bauteile werden erwärmt und dann in heißem Zustand final umgeformt und somit „pressgehärtet“.\n\nvoestalpine Werksmarken\n\n/phs-ultraform 2000\n\n/phs-ultraform 1500\n\n/phs-ultraform 490", "lang": "de"}, {"value": "The “phs components” product group (phs = press-hardened steel) consists of high-strength finished components. The specific characteristics of this product group are exceptional forming possibilities combined with high strength. This declaration summarizes the different processing variants at various voestalpine Metal Forming Division production sites. \n\n“phs-ultraform” is a registered trademark of voestalpine Stahl GmbH. \n\nphs-ultraform (EUIPO registration numbers 013290044 and 005772165): cold-formed components are heated and then formed in a hot state. The material is hardened in the press with the help of cooled dies (press-hardened). \n\n\nvoestalpine trademarks \n\n/phs-ultraform 2000 \n\n/phs-ultraform 1500 \n\n/phs-ultraform 490", "lang": "en"}]}, "quantitativeReference": {"referenceToReferenceFlow": [0]}, "time": {"referenceYear": 2021, "dataSetValidUntil": 2026, "other": {"anies": [{"name": "publicationDateOfEPD", "value": 1626912000000}]}}, "geography": {"locationOfOperationSupplyOrProduction": {"location": "GLO"}}, "technology": {"technologyDescriptionAndIncludedProcesses": [{"value": "Das Ausgangsmaterial für die Herstellung des feuerverzinkten Bandes ist Rohstahl, der über die Primärroute (Hochofen, LD- Stahlwerk) hergestellt wird. Der flüssige Rohstahl wird mittels Stranggussverfahren zu Brammen gegossen. Die gegossenen Brammen werden über Stoß- bzw. Hubbalkenöfen erneut auf 1100-1250 °C erwärmt und in mehreren Walzschritten zu Bändern mit einer Dicke von 1,2-4 mm gewalzt. Auf dem Warmband bildet sich eine Walzzunderschicht aus, die vor der Weiterverarbeitung im Kaltwalzwerk entfernt wird (Entzundern). Dieser Produktionsschritt verläuft zuerst durch eine mechanische Lockerung der Zunderschicht (Streckrichtanlage). In weiterer Folge wird das Stahlband mittels Salz- und Schwefelsäure gebeizt. „phs“ (=press hardening steel) umfasst das Umformen von verzinktem Flachstahl in heißem Zustand. Damit wird dem Ziel von hohen Umformgraden bei gleichzeitig höchsten Festigkeiten Rechnung getragen. Das indirekte Verfahren, „phs-ultraform“: Ausgehend von einem Stahlband oder einer lasergeschweißten Stahlplatine erfolgt die Kaltumformung der Teile in einer hydraulischen oder mechanischen Presse (hohe Maßgenauigkeit). Danach werden die umgeformten Teile auf etwa 900 °C erhitzt und unmittelbar danach in heißem Zustand nochmals gepresst. Durch die gekühlten Werkzeuge erfolgt eine Aufhärtung des Bauteils, die Zinkschicht wird aufgrund der geringeren Umformgrade nicht beschädigt. Das Bauteil wird danach gereinigt. \nTechnische Daten: \nMaßgebend sind die in der Leistungserklärung aufgeführten Daten. \n\nBautechnische Daten: \n\nBlechdicken: von 0,7 bis 3,0 mm\n\nBauteilmasse: von 2 bis 20 kg \n\nBauteilabmessungen: \n\nDie Bauteildimension ist in einem CAD-Modell definiert. Die Abmessungen von typischen phs-Bauteilen von Automotive-Anwendungen reichen von  \n\nBreite: von 70 bis 2000 mm \n\nHöhe: von 20 bis 400 mm \n\nLänge: von 200 bis 3500 mm\n\n\nProduktnormen: \n\nLeistungswerte des Produkts entsprechend der Leistungserklärung in Bezug auf dessen wesentliche Merkmale gemäß \n\nDIN EN 10143:2006, Kontinuierlich schmelztauchveredeltes Band und Blech aus Stahl; Grenzabmaße und Formtoleranzen. \n\nDIN EN 10346:2015, Kontinuierlich schmelztauchveredelte Flacherzeugnisse aus Stahl zum Kaltumformen - Technische Lieferbedingungen. \n\nDIN EN 10338:2015, Warmgewalzte und kaltgewalzte Flacherzeugnisse ohne Überzug aus Mehrphasenstählen zum Kaltumformen - Technische Lieferbedingungen. \n\nSEW 022, 2010, Kontinuierlich schmelztauchveredelte Flacherzeugnisse aus Stahl - Zink-Magnesium Überzüge - Technische Lieferbedingungen. \n\nVDA Werkstoffblatt 239-100, 2016, Flacherzeugnisse aus Stahl zur Kaltumformung. \n\nDie voestalpine Gruppe hält zahlreiche Patente im Zusammenhang mit phs-ultraform. Dies umfasst beispielsweise:\n\nspezielle phs-ultraform gefertigte Bauteile (z. B. TPP)\nOberflächenkonditionierung wie Reinigungsverfahren oder Vorbehandlung\nProzessführung bei der Erwärmung als auch Abkühlung (Vorkühlung) der Bauteile im Presshärteverfahren\nWarmumformwerkzeuge inkl. der Gestaltung von z. B. Kühlkanälen \nDeklarierte Einheit: \nDie vorliegende Umwelt-Produktdeklaration für voestalpine phs-Bauteile bezieht sich auf eine deklarierte Einheit von 1 t pressgehärtete Stahlbauteile.", "lang": "de"}, {"value": "The starting material for the production of hot-dip galvanized strip at voestalpine is crude steel made in the integrated route (blast furnace, LD steelmaking plant) at the Linz site. The liquid crude steel is cast into slabs using a continuous casting method. After cooling, the slabs are reheated in pusher-type or walking beam furnaces to a temperature ranging between 1100 and 1250 °C and rolled in several rolling steps to strips in thicknesses ranging between 1.2 and 4 mm. A mill scale layer forms on the hot-rolled strip and is removed before further processing in the cold-rolling mill (scale removal). This production step first features a mechanical loosening of the scale layer (leveling line). The steel strip is subsequently pickled with hydrochloric and sulfuric acid. “phs” (press hardened steel) consists of hot forming galvanized flat steel. This meets the objective of achieving maximum formability combined with maximum strength. The indirect method, “phs-ultraform”: Starting with a steel strip or a laser-welded steel blank, parts are cold-formed in a hydraulic or mechanical press (high dimensional accuracy). The formed parts are then heated to roughly 900 °C and immediately press-hardened again while they are hot. The cooled dies harden the component, and the low degree of forming prevents the zinc layer from being damaged. The component is then cleaned. \nTechnical data: \nThe data in the Declaration of Performance apply.\n\nStructural data: \n\nThickness of the sheet: 0.7 to 3.0 mm \n\nMass of the component: 2 to 20 kg \n\nComponent dimensions:  \n\nComponent dimensions are defined in a CAD model. \n\n\n\nDimensions of typical phs components for automotive applications:  \n\nWidth: 70 to 2000 mm \n\nHeight: 20 to 400 mm \n\nLength: 200 to 3500 mm \nDeclared unit: \nThis environmental product declaration for voestalpine phs-components refers to a declared unit of 1 t press-hardened steel components.", "lang": "en"}], "technologicalApplicability": [{"value": "phs-Bauteile finden zurzeit vor allem in der Automotive-Industrie Anwendung. Eine Anwendung für andere Branchen mit hohen Anforderungen an Umformgrade, geringes Gewicht und hohe Festigkeit ist möglich. Die vorliegende Analyse erfolgte ausschließlich für phs-Bauteile im automotiven Sektor. \n\nphs-Bauteile werden im überwiegenden Maße für Strukturteile des Chassis verwendet: \n\nLängsträger vorne und hinten\nStoßfängerträger\nSchweller\nQuerträger\nA-Säule\nB-Säule\nDachrahmen  \n\nIn der Regel bestehen Bauteilgruppen (z. B. Längsträger) aus mehreren Einzelbauteilen, die durch entsprechende Fügetechnologie (Schweißen, Kleben, Nieten) miteinander verbunden werden. So können auf die Belastungssituation im Fertigbauteil optimierte Anwendungen realisiert werden.\n\nMit sogenannten „Tailored Property Parts“ (TPP) werden die Bauteileigenschaften „maßgeschneidert“. Durch Zusammenfügen von Flachstahl verschiedener Dicke und Stahlgüte („Laser Welded Blanks“), abschnittsweises Härten und Verstärken von Bauteilsegmenten werden sehr spezifische Anforderungen in Hinblick auf Crashverhalten, Verformbarkeit, Insassenschutz und Energieaufnahme realisiert.\n\n\nEinsatz von pressgehärteten (phs) und TPP-Teilen\n\n\nVerschiedene Varianten von „Tailored Property Parts“", "lang": "de"}, {"value": "phs components are used primarily in the automotive industry. They can also be used in other industries where a high degree of formability, low weight, and high strength are required. The analysis presented here was carried out exclusively for phs components in the automotive sector. phs components are predominantly used for structural chassis components: \nFront and rear side members \nBumper supports \nSills \nCrossmembers \nA pillars \nB pillars \nRoof frames \n\nComponent groups such as side members usually consist of several individual components that are joined together using appropriate joining technologies (welding, bonding, riveting). This makes it possible to optimize applications for load situation in the finished component.\n\n Tailored-property parts (TPP) are used to customize component properties. Very specific characteristics with respect to crash behavior, deformability, occupant protection and energy absorption can be achieved by joining flat steels with different thicknesses and steel grades (“laser-welded blanks”) and by hardening and strengthening sections of component segments. \n\n\nUse of press-hardened steel (phs) and TPP parts\n\n\n\nVariants of tailored-property parts", "lang": "en"}]}}, "modellingAndValidation": {"LCIMethodAndAllocation": {"typeOfDataSet": "EPD", "referenceToLCAMethodDetails": [{"shortDescription": [{"value": "Dünnwandige Profile und Profiltafeln aus Metall.pdf", "lang": "de"}], "type": "source data set", "refObjectId": "b3b18821-5ab5-49b4-84a4-7b931468c986"}], "other": {"anies": [{"name": "subType", "value": "average dataset"}]}}, "dataSourcesTreatmentAndRepresentativeness": {"referenceToDataSource": [{"shortDescription": [{"value": "GaBi Database (all versions)", "lang": "de"}], "type": "source data set", "refObjectId": "28d74cc0-db8b-4d7e-bc44-5f6d56ce0c4a"}, {"shortDescription": [{"value": "GaBi Database Edition 2021, CUP 2021.01", "lang": "de"}], "type": "source data set", "refObjectId": "1cece811-7501-44d4-8067-9259bd5cb835"}], "useAdviceForDataSet": [{"value": "Gültigkeitsbereich: \nDie vorliegende Umwelt-Produktdeklaration gilt für voestalpine phs-ultraform-Bauteile und bezieht sich auf die durchschnittliche Jahresproduktion der betrachteten Standorte bezogen auf 1 t durchschnittliches phs-Bauteil.\n\nDie betrachteten Standorte sind:\n\nvoestalpine Automotive Components Schmölln GmbH (DE),\n voestalpine Automotive Components Schwäbisch Gmünd GmbH & Co. KG (DE)\nvoestalpine Automotive Components Cartersville Inc. (USA)\nvoestalpine Automotive Components Shenyang Co., Ltd. (CN) \nSystemgrenze: \nDie Ökobilanz der durchschnittlichen phs-Bauteile beinhaltet eine cradle-to-gate-Betrachtung (Wiege bis zum Werkstor) der auftretenden Umweltwirkungen mit den Modulen C1-C4 und Modul D (A1-A3 + C + D). Die folgenden Lebenszyklusphasen werden in der Analyse berücksichtigt: \n\nModul A1-A3 | Produktionsstadium \n\nDas Produktionsstadium beinhaltet die Aufwendungen des Herstellungsprozesses der phs-Bauteile an den Standorten Schwäbisch-Gmünd, Schmölln, Shenyang und Cartersville. Dabei wird der indirekte Presshärteprozess zur Produktion von hoch korrosionsbeständigen Leichtbauteilen im jeweiligen Werk abgebildet. Das Vormaterial wird vom integrierten Stahlwerk der voestalpine Standort Linz und der voestalpine Automotive Components Linz angeliefert. Die Bereitstellung der elektrischen Energie erfolgt jeweils vom nationalen Stromnetz. Für die thermische Energie wird Erdgas als Energieträger eingesetzt. Der Ladungsträger variiert gemäß Kundenanforderung und ist nicht in der Deklaration enthalten. \n\nModul C1 | Ausbau \n\nphs-Bauteile werden im Automotiv-Bereich eingesetzt. Die Verwertung der phs-Bauteile erfolgt beim Entsorger. \n\nModul C2 | Transport zur Abfallbehandlung  \n\nModul C2 beinhaltet den Transport zur Abfallbehandlung. Dazu wird der Transport via LKW über 50 km Transportdistanz als repräsentatives Szenario angesetzt.\n\nModul C3 | Abfallbehandlung \n\nDas Fahrzeug wird beim Entsorger in die Grundkomponenten zerlegt und anschließend geschreddert. Nach der Zerkleinerung und Sortierung erreicht der Schrott das Ende der Abfalleigenschaft in C3 und erreicht das Modul D zum Recycling. Aufwendungen für die Zerkleinerung und Sortierung des Stahlschrottes sind aufgrund der Geringfügigkeit der zu erwartenden Umweltwirkung nicht enthalten. Modul C4 | Entsorgung \n\nDas Modul C4 deklariert die durch die Deponierung \n\n(5 % des Produktes) entstehenden Umweltwirkungen. \nModul D | Potenziale und Lasten außerhalb der Systemgrenzen \n\nIm Modul D werden die Substitutionspotenziale von Primärstahl durch ein Recyclingszenario (95 % des \n\nProduktes) dargestellt.", "lang": "de"}, {"value": "Scope: \nThis EPD applies to voestalpine phs-ultraform components. It is based on the average annual production of the sites considered and relates to 1 t average phs-components. \n\nThe results are representative for the following sites:\n\nvoestalpine Automotive Components Schmölln GmbH (DE),\n voestalpine Automotive Components Schwäbisch Gmünd GmbH & Co. KG (DE)\nvoestalpine Automotive Components Cartersville Inc. (USA)\nvoestalpine Automotive Components Shenyang Co., Ltd. (CN) \nSystem boundary: \nThe life cycle assessment of phs-components produced by voestalpine refers to a cradle-to-gate analysis with modules C1-C4 and D (A1-A3 + C + D). The following life cycle phases are taken into consideration in the analysis:\n\nModule A1-A3 | Production stage \n\nThe production stage includes the manufacturing process of the phs- components at the sites in Schwäbisch-Gmünd, Schmölln, Shenyang and Cartersville. Indirect press-hardening for the production of highly corrosion-resistant lightweight components is assessed based on data collected for the Group's plants. The raw material is delivered from the integrated steelworks of voestalpine Linz and voestalpine Automotive Components Linz. Electrical energy is provided by the national power grid and thermal energy provision is based on natural gas. \n\nLoad carriers vary according to customer requirements and is not included in the declaration. \n\n\nModule C1 | Deconstruction and demolition \n\nphs-components are used in the automotive sector. The phs-components are disposed of by the waste management company.\n\nModule C2 | Transport  \n\nThe transport to the disposal of the material is estimated declaring a 50 km radius to waste processing. \n\nModule C3 | Waste treatment \n\nThe vehicle is dismantled into its basic components at the disposal company and shredded. After shredding and sorting, the scrap reaches the end-of-waste status in C3 and reaches module D for recycling. Environmental impacts from shredding and sorting of the steel scrap are not included due to the insignificance of the expected impact.\n\nModule C4 | Disposal  \nModule C4 refers to the emissions from the disposal of the losses from waste processing. The chosen scenario, therefore, includes the environmental burdens of landfilling of 5 % of the material.\n\nModule D | Credits and loads beyond the system boundary\n\nModule D declares the recycling of the recovered steel (95 % of the product). It includes the potential for substituting primary steel.", "lang": "en"}], "other": {"anies": [{"name": "referenceToOriginalEPD", "value": {"shortDescription": {"value": "Warmumgeformte Stahlpressteile (\"phs-ultraform\").pdf", "defaultValue": "Warmumgeformte Stahlpressteile (\"phs-ultraform\").pdf", "lstrings": [{"lang": "de", "value": "Warmumgeformte Stahlpressteile (\"phs-ultraform\").pdf"}]}, "type": "source data set", "uuid": {"uuid": "c8eb4cb1-5cc3-4e5b-9a9f-185510453a83"}, "refObjectId": "c8eb4cb1-5cc3-4e5b-9a9f-185510453a83", "resourceURLs": ["https://oekobaudat.de/OEKOBAU.DAT/resource/sources/c8eb4cb1-5cc3-4e5b-9a9f-185510453a83/Warmumgeformte_Stahlpressteile_phs-ultraform__14402.pdf?version=00.01.000"]}}]}}, "validation": {"review": [{"referenceToNameOfReviewerAndInstitution": [{"shortDescription": [{"value": "Institut Bauen und Umwelt e. V.", "lang": "de"}], "type": "contact data set", "refObjectId": "d111dbec-b024-4be5-86c5-752d6eb2cf95", "uri": "../contacts/d111dbec-b024-4be5-86c5-752d6eb2cf95.xml"}], "type": "Accredited third party review"}]}, "complianceDeclarations": {"compliance": [{"referenceToComplianceSystem": {"shortDescription": [{"value": "DIN EN 15804+A2", "lang": "de"}], "type": "source data set", "refObjectId": "c0016b33-8cf7-415c-ac6e-deba0d21440d", "uri": "../sources/c0016b33-8cf7-415c-ac6e-deba0d21440d.xml"}}, {"referenceToComplianceSystem": {"shortDescription": [{"value": "ISO 14025", "lang": "de"}], "type": "source data set", "refObjectId": "4f2eb655-6e44-4874-a95a-e28f5442cd4d", "uri": "../sources/4f2eb655-6e44-4874-a95a-e28f5442cd4d.xml"}}]}}, "administrativeInformation": {"commissionerAndGoal": {"referenceToCommissioner": [{"shortDescription": [{"value": "voestalpine AG", "lang": "de"}], "type": "contact data set", "refObjectId": "eef08a78-bb8b-429e-a968-c40f32a49ec7", "uri": "../contacts/eef08a78-bb8b-429e-a968-c40f32a49ec7.xml"}]}, "dataGenerator": {"referenceToPersonOrEntityGeneratingTheDataSet": [{"shortDescription": [{"value": "Daxner & Merl GmbH", "lang": "de"}], "type": "contact data set", "refObjectId": "ad8ad627-3991-42b7-a7ca-5a3fe0a34c28", "uri": "../contacts/ad8ad627-3991-42b7-a7ca-5a3fe0a34c28.xml"}]}, "dataEntryBy": {"timeStamp": 1626974531526, "referenceToDataSetFormat": [{"shortDescription": [{"value": "ILCD Format", "lang": "de"}], "type": "source data set", "refObjectId": "a97a0155-0234-4b87-b4ce-a45da52f2a40", "uri": "../sources/a97a0155-0234-4b87-b4ce-a45da52f2a40.xml"}, {"shortDescription": [{"value": "EPD-Datenformaterweiterungen v1.2", "lang": "de"}, {"value": "EPD Data Format Extensions v1.2", "lang": "en"}], "type": "source data set", "refObjectId": "a29449fd-aa2f-4de8-b5d7-4b06b43c6fde", "uri": "../sources/a29449fd-aa2f-4de8-b5d7-4b06b43c6fde.xml"}]}, "publicationAndOwnership": {"dataSetVersion": "00.02.000", "referenceToRegistrationAuthority": {"shortDescription": [{"value": "Institut Bauen und Umwelt e. V.", "lang": "de"}], "type": "contact data set", "refObjectId": "d111dbec-b024-4be5-86c5-752d6eb2cf95", "uri": "../contacts/d111dbec-b024-4be5-86c5-752d6eb2cf95.xml"}, "registrationNumber": "EPD-VOE-20210174-IBB1-DE", "referenceToOwnershipOfDataSet": {"shortDescription": [{"value": "voestalpine AG", "lang": "de"}], "type": "contact data set", "refObjectId": "eef08a78-bb8b-429e-a968-c40f32a49ec7", "uri": "../contacts/eef08a78-bb8b-429e-a968-c40f32a49ec7.xml"}, "copyright": true, "licenseType": "Free of charge for all users and uses", "accessRestrictions": [{"value": "None", "lang": "en"}], "other": {"anies": [{"name": "referenceToPublisher", "value": {"shortDescription": [{"value": "Institut Bauen und Umwelt e. V.", "lang": "de"}], "type": "contact data set", "refObjectId": "d111dbec-b024-4be5-86c5-752d6eb2cf95", "uri": "../contacts/d111dbec-b024-4be5-86c5-752d6eb2cf95.xml"}}]}}}, "exchanges": {"exchange": [{"dataSetInternalID": 0, "referenceToFlowDataSet": {"shortDescription": [{"value": "phs-Bauteile (phs-Bauteile)", "lang": "de"}], "type": "flow data set", "refObjectId": "2ddfaad2-4ace-e6c7-8e84-f6f9ab2f5b84", "uri": "../flows/2ddfaad2-4ace-e6c7-8e84-f6f9ab2f5b84.xml"}, "meanAmount": 1000.0, "referencesToDataSource": {}, "referenceFlow": true, "resolvedFlowVersion": "00.02.000", "resultingflowAmount": 1000.0, "flowProperties": [{"name": [{"lang": "en", "value": "Mass"}, {"lang": "de", "value": "Masse"}], "uuid": "93a60a56-a3c8-11da-a746-0800200b9a66", "referenceFlowProperty": true, "meanValue": 1.0, "referenceUnit": "kg", "unitGroupUUID": "ad38d542-3fe9-439d-9b95-2f5f7752acaf"}], "materialProperties": [{"name": "conversion factor to 1 kg", "value": "0.001", "unit": "-", "unitDescription": "Without unit"}], "typeOfFlow": "Product flow", "classification": {"classHierarchy": "Metalle / Stahl und Eisen / Stahlbleche", "name": "OEKOBAU.DAT"}}, {"dataSetInternalID": 1, "referenceToFlowDataSet": {"shortDescription": [{"value": "Erneuerbare Primärenergie als Energieträger (PERE)", "lang": "de"}, {"value": "Renewable primary energy as energy carrier (PERE)", "lang": "en"}], "type": "flow data set", "refObjectId": "20f32be5-0398-4288-9b6d-accddd195317", "uri": "../flows/20f32be5-0398-4288-9b6d-accddd195317.xml"}, "exchange direction": "INPUT", "other": {"anies": [{"name": "referenceToUnitGroupDataSet", "value": {"shortDescription": [{"value": "MJ", "lang": "de"}], "type": "unit group data set", "refObjectId": "93a60a57-a3c8-11da-a746-0800200c9a66", "uri": "../unitgroups/93a60a57-a3c8-11da-a746-0800200c9a66.xml"}}, {"value": "4336.63614425174", "module": "A1-A3"}, {"value": "0", "module": "C1"}, {"value": "2.29162705358998", "module": "C2"}, {"value": "0", "module": "C3"}, {"value": "2.56802636768431", "module": "C4"}, {"value": "1851.84620186446", "module": "D"}]}, "resolvedFlowVersion": "38.00.000", "flowProperties": [], "typeOfFlow": "Other flow", "classification": {"classHierarchy": "Quantities", "name": "GaBiCategories"}}, {"dataSetInternalID": 2, "referenceToFlowDataSet": {"shortDescription": [{"value": "Erneuerbare Primärenergie zur stofflichen Nutzung (PERM)", "lang": "de"}, {"value": "Renewable primary energy resources as material utilization (PERM)", "lang": "en"}], "type": "flow data set", "refObjectId": "fb3ec0de-548d-4508-aea5-00b73bf6f702", "uri": "../flows/fb3ec0de-548d-4508-aea5-00b73bf6f702.xml"}, "exchange direction": "INPUT", "other": {"anies": [{"name": "referenceToUnitGroupDataSet", "value": {"shortDescription": [{"value": "MJ", "lang": "de"}], "type": "unit group data set", "refObjectId": "93a60a57-a3c8-11da-a746-0800200c9a66", "uri": "../unitgroups/93a60a57-a3c8-11da-a746-0800200c9a66.xml"}}, {"value": "0", "module": "A1-A3"}, {"value": "0", "module": "C1"}, {"value": "0", "module": "C2"}, {"value": "0", "module": "C3"}, {"value": "0", "module": "C4"}, {"value": "0", "module": "D"}]}, "resolvedFlowVersion": "38.00.000", "flowProperties": [], "typeOfFlow": "Other flow", "classification": {"classHierarchy": "Quantities", "name": "GaBiCategories"}}, {"dataSetInternalID": 3, "referenceToFlowDataSet": {"shortDescription": [{"value": "Total erneuerbare Primärenergie (PERT)", "lang": "de"}, {"value": "Total use of renewable primary energy resources (PERT)", "lang": "en"}], "type": "flow data set", "refObjectId": "53f97275-fa8a-4cdd-9024-65936002acd0", "uri": "../flows/53f97275-fa8a-4cdd-9024-65936002acd0.xml"}, "exchange direction": "INPUT", "other": {"anies": [{"name": "referenceToUnitGroupDataSet", "value": {"shortDescription": [{"value": "MJ", "lang": "de"}], "type": "unit group data set", "refObjectId": "93a60a57-a3c8-11da-a746-0800200c9a66", "uri": "../unitgroups/93a60a57-a3c8-11da-a746-0800200c9a66.xml"}}, {"value": "4336.63614425174", "module": "A1-A3"}, {"value": "0", "module": "C1"}, {"value": "2.29162705358998", "module": "C2"}, {"value": "0", "module": "C3"}, {"value": "2.56802636768431", "module": "C4"}, {"value": "1851.84620186446", "module": "D"}]}, "resolvedFlowVersion": "38.00.000", "flowProperties": [], "typeOfFlow": "Other flow", "classification": {"classHierarchy": "Quantities / Environmental quantities / EPD EN 15804 / LCI indicators", "name": "GaBiCategories"}}, {"dataSetInternalID": 4, "referenceToFlowDataSet": {"shortDescription": [{"value": "Nicht-erneuerbare Primärenergie als Energieträger (PENRE)", "lang": "de"}, {"value": "Non renewable primary energy as energy carrier (PENRE)", "lang": "en"}], "type": "flow data set", "refObjectId": "ac857178-2b45-46ec-892a-a9a4332f0372", "uri": "../flows/ac857178-2b45-46ec-892a-a9a4332f0372.xml"}, "exchange direction": "INPUT", "other": {"anies": [{"name": "referenceToUnitGroupDataSet", "value": {"shortDescription": [{"value": "MJ", "lang": "de"}], "type": "unit group data set", "refObjectId": "93a60a57-a3c8-11da-a746-0800200c9a66", "uri": "../unitgroups/93a60a57-a3c8-11da-a746-0800200c9a66.xml"}}, {"value": "48958.1660913311", "module": "A1-A3"}, {"value": "0", "module": "C1"}, {"value": "39.9699776934577", "module": "C2"}, {"value": "0", "module": "C3"}, {"value": "35.560110058703", "module": "C4"}, {"value": "-20141.2141064983", "module": "D"}]}, "resolvedFlowVersion": "38.00.000", "flowProperties": [], "typeOfFlow": "Other flow", "classification": {"classHierarchy": "Quantities", "name": "GaBiCategories"}}, {"dataSetInternalID": 5, "referenceToFlowDataSet": {"shortDescription": [{"value": "Nicht-erneuerbare Primärenergie zur stofflichen Nutzung (PENRM)", "lang": "de"}, {"value": "Non renewable primary energy as material utilization (PENRM)", "lang": "en"}], "type": "flow data set", "refObjectId": "1421caa0-679d-4bf4-b282-0eb850ccae27", "uri": "../flows/1421caa0-679d-4bf4-b282-0eb850ccae27.xml"}, "exchange direction": "INPUT", "other": {"anies": [{"name": "referenceToUnitGroupDataSet", "value": {"shortDescription": [{"value": "MJ", "lang": "de"}], "type": "unit group data set", "refObjectId": "93a60a57-a3c8-11da-a746-0800200c9a66", "uri": "../unitgroups/93a60a57-a3c8-11da-a746-0800200c9a66.xml"}}, {"value": "0", "module": "A1-A3"}, {"value": "0", "module": "C1"}, {"value": "0", "module": "C2"}, {"value": "0", "module": "C3"}, {"value": "0", "module": "C4"}, {"value": "0", "module": "D"}]}, "resolvedFlowVersion": "38.00.000", "flowProperties": [], "typeOfFlow": "Other flow", "classification": {"classHierarchy": "Quantities", "name": "GaBiCategories"}}, {"dataSetInternalID": 6, "referenceToFlowDataSet": {"shortDescription": [{"value": "Total nicht erneuerbare Primärenergie (PENRT)", "lang": "de"}, {"value": "Total use of non renewable primary energy resources (PENRT)", "lang": "en"}], "type": "flow data set", "refObjectId": "06159210-646b-4c8d-8583-da9b3b95a6c1", "uri": "../flows/06159210-646b-4c8d-8583-da9b3b95a6c1.xml"}, "exchange direction": "INPUT", "other": {"anies": [{"name": "referenceToUnitGroupDataSet", "value": {"shortDescription": [{"value": "MJ", "lang": "de"}], "type": "unit group data set", "refObjectId": "93a60a57-a3c8-11da-a746-0800200c9a66", "uri": "../unitgroups/93a60a57-a3c8-11da-a746-0800200c9a66.xml"}}, {"value": "48958.1660913311", "module": "A1-A3"}, {"value": "0", "module": "C1"}, {"value": "39.9699776934577", "module": "C2"}, {"value": "0", "module": "C3"}, {"value": "35.560110058703", "module": "C4"}, {"value": "-20141.2141064983", "module": "D"}]}, "resolvedFlowVersion": "38.00.000", "flowProperties": [], "typeOfFlow": "Other flow", "classification": {"classHierarchy": "Quantities / Environmental quantities / EPD EN 15804 / LCI indicators", "name": "GaBiCategories"}}, {"dataSetInternalID": 7, "referenceToFlowDataSet": {"shortDescription": [{"value": "Einsatz von Sekundärstoffen (SM)", "lang": "de"}, {"value": "Use of secondary material (SM)", "lang": "en"}], "type": "flow data set", "refObjectId": "c6a1f35f-2d09-4f54-8dfb-97e502e1ce92", "uri": "../flows/c6a1f35f-2d09-4f54-8dfb-97e502e1ce92.xml"}, "exchange direction": "INPUT", "other": {"anies": [{"name": "referenceToUnitGroupDataSet", "value": {"shortDescription": [{"value": "kg", "lang": "de"}], "type": "unit group data set", "refObjectId": "ad38d542-3fe9-439d-9b95-2f5f7752acaf", "uri": "../unitgroups/ad38d542-3fe9-439d-9b95-2f5f7752acaf.xml"}}, {"value": "221.511526635832", "module": "A1-A3"}, {"value": "0", "module": "C1"}, {"value": "0", "module": "C2"}, {"value": "0", "module": "C3"}, {"value": "0", "module": "C4"}, {"value": "1364.39", "module": "D"}]}, "resolvedFlowVersion": "38.00.000", "flowProperties": [], "typeOfFlow": "Other flow", "classification": {"classHierarchy": "Quantities / Environmental quantities / EPD EN 15804 / LCI indicators", "name": "GaBiCategories"}}, {"dataSetInternalID": 8, "referenceToFlowDataSet": {"shortDescription": [{"value": "Erneuerbare Sekundärbrennstoffe (RSF)", "lang": "de"}, {"value": "Use of renewable secondary fuels (RSF)", "lang": "en"}], "type": "flow data set", "refObjectId": "64333088-a55f-4aa2-9a31-c10b07816787", "uri": "../flows/64333088-a55f-4aa2-9a31-c10b07816787.xml"}, "exchange direction": "INPUT", "other": {"anies": [{"name": "referenceToUnitGroupDataSet", "value": {"shortDescription": [{"value": "MJ", "lang": "de"}], "type": "unit group data set", "refObjectId": "93a60a57-a3c8-11da-a746-0800200c9a66", "uri": "../unitgroups/93a60a57-a3c8-11da-a746-0800200c9a66.xml"}}, {"value": "0", "module": "A1-A3"}, {"value": "0", "module": "C1"}, {"value": "0", "module": "C2"}, {"value": "0", "module": "C3"}, {"value": "0", "module": "C4"}, {"value": "0", "module": "D"}]}, "resolvedFlowVersion": "38.00.000", "flowProperties": [], "typeOfFlow": "Other flow", "classification": {"classHierarchy": "Quantities / Environmental quantities / EPD EN 15804 / LCI indicators", "name": "GaBiCategories"}}, {"dataSetInternalID": 9, "referenceToFlowDataSet": {"shortDescription": [{"value": "Nicht erneuerbare Sekundärbrennstoffe (NRSF)", "lang": "de"}, {"value": "Use of non renewable secondary fuels (NRSF)", "lang": "en"}], "type": "flow data set", "refObjectId": "89def144-d39a-4287-b86f-efde453ddcb2", "uri": "../flows/89def144-d39a-4287-b86f-efde453ddcb2.xml"}, "exchange direction": "INPUT", "other": {"anies": [{"name": "referenceToUnitGroupDataSet", "value": {"shortDescription": [{"value": "MJ", "lang": "de"}], "type": "unit group data set", "refObjectId": "93a60a57-a3c8-11da-a746-0800200c9a66", "uri": "../unitgroups/93a60a57-a3c8-11da-a746-0800200c9a66.xml"}}, {"value": "0", "module": "A1-A3"}, {"value": "0", "module": "C1"}, {"value": "0", "module": "C2"}, {"value": "0", "module": "C3"}, {"value": "0", "module": "C4"}, {"value": "0", "module": "D"}]}, "resolvedFlowVersion": "38.00.000", "flowProperties": [], "typeOfFlow": "Other flow", "classification": {"classHierarchy": "Quantities / Environmental quantities / EPD EN 15804 / LCI indicators", "name": "GaBiCategories"}}, {"dataSetInternalID": 10, "referenceToFlowDataSet": {"shortDescription": [{"value": "Einsatz von Süßwasserressourcen (FW)", "lang": "de"}, {"value": "Use of net fresh water (FW)", "lang": "en"}], "type": "flow data set", "refObjectId": "3cf952c8-f3a4-461d-8c96-96456ca62246", "uri": "../flows/3cf952c8-f3a4-461d-8c96-96456ca62246.xml"}, "exchange direction": "INPUT", "other": {"anies": [{"name": "referenceToUnitGroupDataSet", "value": {"shortDescription": [{"value": "m^3", "lang": "de"}], "type": "unit group data set", "refObjectId": "cd950537-0a98-4044-9ba7-9f9a68d0a504", "uri": "../unitgroups/cd950537-0a98-4044-9ba7-9f9a68d0a504.xml"}}, {"value": "11.4967869925863", "module": "A1-A3"}, {"value": "0", "module": "C1"}, {"value": "0.00262465508256471", "module": "C2"}, {"value": "0", "module": "C3"}, {"value": "0.000367450889833254", "module": "C4"}, {"value": "-10.1947018513312", "module": "D"}]}, "resolvedFlowVersion": "38.00.000", "flowProperties": [], "typeOfFlow": "Other flow", "classification": {"classHierarchy": "Quantities / Environmental quantities / EPD EN 15804 / LCI indicators", "name": "GaBiCategories"}}, {"dataSetInternalID": 11, "referenceToFlowDataSet": {"shortDescription": [{"value": "Gefährlicher Abfall zur Deponie (HWD)", "lang": "de"}, {"value": "Hazardous waste disposed (HWD)", "lang": "en"}], "type": "flow data set", "refObjectId": "430f9e0f-59b2-46a0-8e0d-55e0e84948fc", "uri": "../flows/430f9e0f-59b2-46a0-8e0d-55e0e84948fc.xml"}, "exchange direction": "OUTPUT", "other": {"anies": [{"name": "referenceToUnitGroupDataSet", "value": {"shortDescription": [{"value": "kg", "lang": "de"}], "type": "unit group data set", "refObjectId": "ad38d542-3fe9-439d-9b95-2f5f7752acaf", "uri": "../unitgroups/ad38d542-3fe9-439d-9b95-2f5f7752acaf.xml"}}, {"value": "1.22578408372084E-05", "module": "A1-A3"}, {"value": "0", "module": "C1"}, {"value": "2.10610417494668E-09", "module": "C2"}, {"value": "0", "module": "C3"}, {"value": "6.30055255131535E-09", "module": "C4"}, {"value": "5.61630635117804E-06", "module": "D"}]}, "resolvedFlowVersion": "38.00.000", "flowProperties": [], "typeOfFlow": "Other flow", "classification": {"classHierarchy": "Quantities / Environmental quantities / EPD EN 15804 / LCI indicators", "name": "GaBiCategories"}}, {"dataSetInternalID": 12, "referenceToFlowDataSet": {"shortDescription": [{"value": "Entsorgter nicht gefährlicher Abfall (NHWD)", "lang": "de"}, {"value": "Non hazardous waste disposed (NHWD)", "lang": "en"}], "type": "flow data set", "refObjectId": "b29ef66b-e286-4afa-949f-62f1a7b4d7fa", "uri": "../flows/b29ef66b-e286-4afa-949f-62f1a7b4d7fa.xml"}, "exchange direction": "OUTPUT", "other": {"anies": [{"name": "referenceToUnitGroupDataSet", "value": {"shortDescription": [{"value": "kg", "lang": "de"}], "type": "unit group data set", "refObjectId": "ad38d542-3fe9-439d-9b95-2f5f7752acaf", "uri": "../unitgroups/ad38d542-3fe9-439d-9b95-2f5f7752acaf.xml"}}, {"value": "51.6285279295263", "module": "A1-A3"}, {"value": "0", "module": "C1"}, {"value": "0.006270810990958", "module": "C2"}, {"value": "0", "module": "C3"}, {"value": "50.0681660982345", "module": "C4"}, {"value": "242.107361550284", "module": "D"}]}, "resolvedFlowVersion": "38.00.000", "flowProperties": [], "typeOfFlow": "Other flow", "classification": {"classHierarchy": "Quantities / Environmental quantities / EPD EN 15804 / LCI indicators", "name": "GaBiCategories"}}, {"dataSetInternalID": 13, "referenceToFlowDataSet": {"shortDescription": [{"value": "Entsorgter radioaktiver Abfall (RWD)", "lang": "de"}, {"value": "Radioactive waste disposed (RWD)", "lang": "en"}], "type": "flow data set", "refObjectId": "3449546e-52ad-4b39-b809-9fb77cea8ff6", "uri": "../flows/3449546e-52ad-4b39-b809-9fb77cea8ff6.xml"}, "exchange direction": "OUTPUT", "other": {"anies": [{"name": "referenceToUnitGroupDataSet", "value": {"shortDescription": [{"value": "kg", "lang": "de"}], "type": "unit group data set", "refObjectId": "ad38d542-3fe9-439d-9b95-2f5f7752acaf", "uri": "../unitgroups/ad38d542-3fe9-439d-9b95-2f5f7752acaf.xml"}}, {"value": "0.714946553528918", "module": "A1-A3"}, {"value": "0", "module": "C1"}, {"value": "7.25025813208313E-05", "module": "C2"}, {"value": "0", "module": "C3"}, {"value": "0.00040531725055476", "module": "C4"}, {"value": "0.000729027289166077", "module": "D"}]}, "resolvedFlowVersion": "38.00.000", "flowProperties": [], "typeOfFlow": "Other flow", "classification": {"classHierarchy": "Quantities / Environmental quantities / EPD EN 15804 / LCI indicators", "name": "GaBiCategories"}}, {"dataSetInternalID": 14, "referenceToFlowDataSet": {"shortDescription": [{"value": "Komponenten für die Wiederverwendung (CRU)", "lang": "de"}, {"value": "Components for re-use (CRU)", "lang": "en"}], "type": "flow data set", "refObjectId": "a2b32f97-3fc7-4af2-b209-525bc6426f33", "uri": "../flows/a2b32f97-3fc7-4af2-b209-525bc6426f33.xml"}, "exchange direction": "OUTPUT", "other": {"anies": [{"name": "referenceToUnitGroupDataSet", "value": {"shortDescription": [{"value": "kg", "lang": "de"}], "type": "unit group data set", "refObjectId": "ad38d542-3fe9-439d-9b95-2f5f7752acaf", "uri": "../unitgroups/ad38d542-3fe9-439d-9b95-2f5f7752acaf.xml"}}, {"value": "0", "module": "A1-A3"}, {"value": "0", "module": "C1"}, {"value": "0", "module": "C2"}, {"value": "0", "module": "C3"}, {"value": "0", "module": "C4"}, {"value": "0", "module": "D"}]}, "resolvedFlowVersion": "38.00.000", "flowProperties": [], "typeOfFlow": "Other flow", "classification": {"classHierarchy": "Quantities / Environmental quantities / EPD EN 15804 / LCI indicators", "name": "GaBiCategories"}}, {"dataSetInternalID": 15, "referenceToFlowDataSet": {"shortDescription": [{"value": "Stoffe zum Recycling (MFR)", "lang": "de"}, {"value": "Materials for recycling (MFR)", "lang": "en"}], "type": "flow data set", "refObjectId": "d7fe48a5-4103-49c8-9aae-b0b5dfdbd6ae", "uri": "../flows/d7fe48a5-4103-49c8-9aae-b0b5dfdbd6ae.xml"}, "exchange direction": "OUTPUT", "other": {"anies": [{"name": "referenceToUnitGroupDataSet", "value": {"shortDescription": [{"value": "kg", "lang": "de"}], "type": "unit group data set", "refObjectId": "ad38d542-3fe9-439d-9b95-2f5f7752acaf", "uri": "../unitgroups/ad38d542-3fe9-439d-9b95-2f5f7752acaf.xml"}}, {"value": "633", "module": "A1-A3"}, {"value": "0", "module": "C1"}, {"value": "0", "module": "C2"}, {"value": "950", "module": "C3"}, {"value": "0", "module": "C4"}, {"value": "0", "module": "D"}]}, "resolvedFlowVersion": "38.00.000", "flowProperties": [], "typeOfFlow": "Other flow", "classification": {"classHierarchy": "Quantities / Environmental quantities / EPD EN 15804 / LCI indicators", "name": "GaBiCategories"}}, {"dataSetInternalID": 16, "referenceToFlowDataSet": {"shortDescription": [{"value": "Stoffe für die Energierückgewinnung (MER)", "lang": "de"}, {"value": "Materials for energy recovery (MER)", "lang": "en"}], "type": "flow data set", "refObjectId": "59a9181c-3aaf-46ee-8b13-2b3723b6e447", "uri": "../flows/59a9181c-3aaf-46ee-8b13-2b3723b6e447.xml"}, "exchange direction": "OUTPUT", "other": {"anies": [{"name": "referenceToUnitGroupDataSet", "value": {"shortDescription": [{"value": "kg", "lang": "de"}], "type": "unit group data set", "refObjectId": "ad38d542-3fe9-439d-9b95-2f5f7752acaf", "uri": "../unitgroups/ad38d542-3fe9-439d-9b95-2f5f7752acaf.xml"}}, {"value": "0", "module": "A1-A3"}, {"value": "0", "module": "C1"}, {"value": "0", "module": "C2"}, {"value": "0", "module": "C3"}, {"value": "0", "module": "C4"}, {"value": "0", "module": "D"}]}, "resolvedFlowVersion": "38.00.000", "flowProperties": [], "typeOfFlow": "Other flow", "classification": {"classHierarchy": "Quantities / Environmental quantities / EPD EN 15804 / LCI indicators", "name": "GaBiCategories"}}, {"dataSetInternalID": 17, "referenceToFlowDataSet": {"shortDescription": [{"value": "Exportierte elektrische Energie (EEE)", "lang": "de"}, {"value": "Exported electrical energy (EEE)", "lang": "en"}], "type": "flow data set", "refObjectId": "4da0c987-2b76-40d6-9e9e-82a017aaaf29", "uri": "../flows/4da0c987-2b76-40d6-9e9e-82a017aaaf29.xml"}, "exchange direction": "OUTPUT", "other": {"anies": [{"name": "referenceToUnitGroupDataSet", "value": {"shortDescription": [{"value": "MJ", "lang": "de"}], "type": "unit group data set", "refObjectId": "93a60a57-a3c8-11da-a746-0800200c9a66", "uri": "../unitgroups/93a60a57-a3c8-11da-a746-0800200c9a66.xml"}}, {"value": "0", "module": "A1-A3"}, {"value": "0", "module": "C1"}, {"value": "0", "module": "C2"}, {"value": "0", "module": "C3"}, {"value": "0", "module": "C4"}, {"value": "0", "module": "D"}]}, "resolvedFlowVersion": "38.00.000", "flowProperties": [], "typeOfFlow": "Other flow", "classification": {"classHierarchy": "Quantities / Environmental quantities / EPD EN 15804 / LCI indicators", "name": "GaBiCategories"}}, {"dataSetInternalID": 18, "referenceToFlowDataSet": {"shortDescription": [{"value": "Exportierte thermische Energie (EET)", "lang": "de"}, {"value": "Exported thermal energy (EET)", "lang": "en"}], "type": "flow data set", "refObjectId": "98daf38a-7a79-46d3-9a37-2b7bd0955810", "uri": "../flows/98daf38a-7a79-46d3-9a37-2b7bd0955810.xml"}, "exchange direction": "OUTPUT", "other": {"anies": [{"name": "referenceToUnitGroupDataSet", "value": {"shortDescription": [{"value": "MJ", "lang": "de"}], "type": "unit group data set", "refObjectId": "93a60a57-a3c8-11da-a746-0800200c9a66", "uri": "../unitgroups/93a60a57-a3c8-11da-a746-0800200c9a66.xml"}}, {"value": "0", "module": "A1-A3"}, {"value": "0", "module": "C1"}, {"value": "0", "module": "C2"}, {"value": "0", "module": "C3"}, {"value": "0", "module": "C4"}, {"value": "0", "module": "D"}]}, "resolvedFlowVersion": "38.00.000", "flowProperties": [], "typeOfFlow": "Other flow", "classification": {"classHierarchy": "Quantities / Environmental quantities / EPD EN 15804 / LCI indicators", "name": "GaBiCategories"}}]}, "LCIAResults": {"LCIAResult": [{"referenceToLCIAMethodDataSet": {"shortDescription": [{"value": "Globales Erwärmungspotenzial total (GWP-total)", "lang": "de"}, {"value": "Global Warming Potential total (GWP-total)", "lang": "en"}], "type": "LCIA method data set", "refObjectId": "6a37f984-a4b3-458a-a20a-64418c145fa2", "uri": "../lciamethods/6a37f984-a4b3-458a-a20a-64418c145fa2.xml"}, "other": {"anies": [{"name": "referenceToUnitGroupDataSet", "value": {"shortDescription": [{"value": "kg CO_(2)-Äq.", "lang": "de"}], "type": "unit group data set", "refObjectId": "1ebf3012-d0db-4de2-aefd-ef30cedb0be1", "uri": "../unitgroups/1ebf3012-d0db-4de2-aefd-ef30cedb0be1.xml"}}, {"value": "4889.41943703268", "module": "A1-A3"}, {"value": "0", "module": "C1"}, {"value": "3.02406984359964", "module": "C2"}, {"value": "0", "module": "C3"}, {"value": "2.41918382472411", "module": "C4"}, {"value": "-2314.48429449992", "module": "D"}]}}, {"referenceToLCIAMethodDataSet": {"shortDescription": [{"value": "Globales Erwärmungspotenzial fossil (GWP-fossil)", "lang": "de"}, {"value": "Global Warming Potential fossil fuels (GWP-fossil)", "lang": "en"}], "type": "LCIA method data set", "refObjectId": "5f635281-343e-44fb-83df-1971b155e6b6", "uri": "../lciamethods/5f635281-343e-44fb-83df-1971b155e6b6.xml"}, "other": {"anies": [{"name": "referenceToUnitGroupDataSet", "value": {"shortDescription": [{"value": "kg CO_(2)-Äq.", "lang": "de"}], "type": "unit group data set", "refObjectId": "1ebf3012-d0db-4de2-aefd-ef30cedb0be1", "uri": "../unitgroups/1ebf3012-d0db-4de2-aefd-ef30cedb0be1.xml"}}, {"value": "4874.8508161572", "module": "A1-A3"}, {"value": "0", "module": "C1"}, {"value": "3.00319194896064", "module": "C2"}, {"value": "0", "module": "C3"}, {"value": "2.44174990564248", "module": "C4"}, {"value": "-2313.32047731488", "module": "D"}]}}, {"referenceToLCIAMethodDataSet": {"shortDescription": [{"value": "Globales Erwärmungspotenzial biogen (GWP-biogenic)", "lang": "de"}, {"value": "Global Warming Potential biogenic (GWP-biogenic)", "lang": "en"}], "type": "LCIA method data set", "refObjectId": "2356e1ab-0185-4db5-86e5-16de51c7485c", "uri": "../lciamethods/2356e1ab-0185-4db5-86e5-16de51c7485c.xml"}, "other": {"anies": [{"name": "referenceToUnitGroupDataSet", "value": {"shortDescription": [{"value": "kg CO_(2)-Äq.", "lang": "de"}], "type": "unit group data set", "refObjectId": "1ebf3012-d0db-4de2-aefd-ef30cedb0be1", "uri": "../unitgroups/1ebf3012-d0db-4de2-aefd-ef30cedb0be1.xml"}}, {"value": "12.094404025729", "module": "A1-A3"}, {"value": "0", "module": "C1"}, {"value": "-0.00356121612494431", "module": "C2"}, {"value": "0", "module": "C3"}, {"value": "-0.0250097349651544", "module": "C4"}, {"value": "-1.49860454363348", "module": "D"}]}}, {"referenceToLCIAMethodDataSet": {"shortDescription": [{"value": "Globales Erwärmungspotenzial luluc (GWP-luluc)", "lang": "de"}, {"value": "Global Warming Potential luluc (GWP-luluc)", "lang": "en"}], "type": "LCIA method data set", "refObjectId": "4331bbdb-978a-490d-8707-eeb047f01a55", "uri": "../lciamethods/4331bbdb-978a-490d-8707-eeb047f01a55.xml"}, "other": {"anies": [{"name": "referenceToUnitGroupDataSet", "value": {"shortDescription": [{"value": "kg CO_(2)-Äq.", "lang": "de"}], "type": "unit group data set", "refObjectId": "1ebf3012-d0db-4de2-aefd-ef30cedb0be1", "uri": "../unitgroups/1ebf3012-d0db-4de2-aefd-ef30cedb0be1.xml"}}, {"value": "2.47421684974959", "module": "A1-A3"}, {"value": "0", "module": "C1"}, {"value": "0.0244391107639501", "module": "C2"}, {"value": "0", "module": "C3"}, {"value": "0.0024436540467793", "module": "C4"}, {"value": "0.33478735859077", "module": "D"}]}}, {"referenceToLCIAMethodDataSet": {"shortDescription": [{"value": "Abbau Potential der stratosphärischen Ozonschicht (ODP)", "lang": "de"}, {"value": "Depletion potential of the stratospheric ozone layer (ODP)", "lang": "en"}], "type": "LCIA method data set", "refObjectId": "b5c629d6-def3-11e6-bf01-fe55135034f3", "uri": "../lciamethods/b5c629d6-def3-11e6-bf01-fe55135034f3.xml"}, "other": {"anies": [{"name": "referenceToUnitGroupDataSet", "value": {"shortDescription": [{"value": "kg CFC11-Äq.", "lang": "de"}], "type": "unit group data set", "refObjectId": "d9e957c9-7309-4474-bf3a-7777df6c4e5b", "uri": "../unitgroups/d9e957c9-7309-4474-bf3a-7777df6c4e5b.xml"}}, {"value": "8.0166751638189E-11", "module": "A1-A3"}, {"value": "0", "module": "C1"}, {"value": "5.90297134895215E-16", "module": "C2"}, {"value": "0", "module": "C3"}, {"value": "5.76801483752193E-15", "module": "C4"}, {"value": "-3.85713117038565E-12", "module": "D"}]}}, {"referenceToLCIAMethodDataSet": {"shortDescription": [{"value": "Versauerungspotenzial von Boden und Wasser (AP)", "lang": "de"}, {"value": "Acidification potential of land and water (AP)", "lang": "en"}], "type": "LCIA method data set", "refObjectId": "b5c611c6-def3-11e6-bf01-fe55135034f3", "uri": "../lciamethods/b5c611c6-def3-11e6-bf01-fe55135034f3.xml"}, "other": {"anies": [{"name": "referenceToUnitGroupDataSet", "value": {"shortDescription": [{"value": "mol H^(+)-Äq.", "lang": "de"}], "type": "unit group data set", "refObjectId": "42e089ac-92bf-4bf2-8ca1-5fc40d18f2ed", "uri": "../unitgroups/42e089ac-92bf-4bf2-8ca1-5fc40d18f2ed.xml"}}, {"value": "13.6488258978728", "module": "A1-A3"}, {"value": "0", "module": "C1"}, {"value": "0.00991631767120498", "module": "C2"}, {"value": "0", "module": "C3"}, {"value": "0.00777562069923066", "module": "C4"}, {"value": "-4.15265308821301", "module": "D"}]}}, {"referenceToLCIAMethodDataSet": {"shortDescription": [{"value": "Eutrophierungspotenzial Süßwasser (EP-freshwater)", "lang": "de"}, {"value": "Eutrophication potential aquatic freshwater (EP-freshwater)", "lang": "en"}], "type": "LCIA method data set", "refObjectId": "b53ec18f-7377-4ad3-86eb-cc3f4f276b2b", "uri": "../lciamethods/b53ec18f-7377-4ad3-86eb-cc3f4f276b2b.xml"}, "other": {"anies": [{"name": "referenceToUnitGroupDataSet", "value": {"shortDescription": [{"value": "kg PO_(4)-Äq.", "lang": "de"}], "type": "unit group data set", "refObjectId": "0429039d-a61d-4590-ba67-aa4a20a810a1", "uri": "../unitgroups/0429039d-a61d-4590-ba67-aa4a20a810a1.xml"}}, {"value": "0.00626299593223431", "module": "A1-A3"}, {"value": "0", "module": "C1"}, {"value": "8.88275548806866E-06", "module": "C2"}, {"value": "0", "module": "C3"}, {"value": "1.8584714056159E-06", "module": "C4"}, {"value": "-0.000473035178161964", "module": "D"}]}}, {"referenceToLCIAMethodDataSet": {"shortDescription": [{"value": "Eutrophierungspotenzial Salzwasser (EP-marine)", "lang": "de"}, {"value": "Eutrophication potential aquatic marine (EP-marine)", "lang": "en"}], "type": "LCIA method data set", "refObjectId": "b5c619fa-def3-11e6-bf01-fe55135034f3", "uri": "../lciamethods/b5c619fa-def3-11e6-bf01-fe55135034f3.xml"}, "other": {"anies": [{"name": "referenceToUnitGroupDataSet", "value": {"shortDescription": [{"value": "kg N-Äq.", "lang": "de"}], "type": "unit group data set", "refObjectId": "d05bb823-ecdf-4686-8c40-bf1d9257859f", "uri": "../unitgroups/d05bb823-ecdf-4686-8c40-bf1d9257859f.xml"}}, {"value": "3.23123757633342", "module": "A1-A3"}, {"value": "0", "module": "C1"}, {"value": "0.004554984082094", "module": "C2"}, {"value": "0", "module": "C3"}, {"value": "0.00193046056746469", "module": "C4"}, {"value": "-0.618879696819431", "module": "D"}]}}, {"referenceToLCIAMethodDataSet": {"shortDescription": [{"value": "Eutrophierungspotenzial Land (EP-terrestrial)", "lang": "de"}, {"value": "Eutrophication potential terrestrial (EP-terrestrial)", "lang": "en"}], "type": "LCIA method data set", "refObjectId": "b5c614d2-def3-11e6-bf01-fe55135034f3", "uri": "../lciamethods/b5c614d2-def3-11e6-bf01-fe55135034f3.xml"}, "other": {"anies": [{"name": "referenceToUnitGroupDataSet", "value": {"shortDescription": [{"value": "mol N-Äq.", "lang": "de"}], "type": "unit group data set", "refObjectId": "71b4d617-0ec9-4d3f-b65e-e438940c2401", "uri": "../unitgroups/71b4d617-0ec9-4d3f-b65e-e438940c2401.xml"}}, {"value": "35.1373723907561", "module": "A1-A3"}, {"value": "0", "module": "C1"}, {"value": "0.0508448603038949", "module": "C2"}, {"value": "0", "module": "C3"}, {"value": "0.0211802245417931", "module": "C4"}, {"value": "-6.03350597899233", "module": "D"}]}}, {"referenceToLCIAMethodDataSet": {"shortDescription": [{"value": "Bildungspotential für troposphärisches Ozon (POCP)", "lang": "de"}, {"value": "Formation potential of tropospheric ozone photochemical oxidants (POCP)", "lang": "en"}], "type": "LCIA method data set", "refObjectId": "b5c610fe-def3-11e6-bf01-fe55135034f3", "uri": "../lciamethods/b5c610fe-def3-11e6-bf01-fe55135034f3.xml"}, "other": {"anies": [{"name": "referenceToUnitGroupDataSet", "value": {"shortDescription": [{"value": "kg NMVOC-Äq.", "lang": "de"}], "type": "unit group data set", "refObjectId": "d27c25f8-fbc1-44c6-b47b-4adbae4199c6", "uri": "../unitgroups/d27c25f8-fbc1-44c6-b47b-4adbae4199c6.xml"}}, {"value": "10.136962510957", "module": "A1-A3"}, {"value": "0", "module": "C1"}, {"value": "0.00894108054228951", "module": "C2"}, {"value": "0", "module": "C3"}, {"value": "0.00608284454471822", "module": "C4"}, {"value": "-3.16844596333714", "module": "D"}]}}, {"referenceToLCIAMethodDataSet": {"shortDescription": [{"value": "Potenzial für den abiotischen Abbau nicht fossiler Ressourcen (ADPE)", "lang": "de"}, {"value": "Abiotic depletion potential for non fossil resources (ADPE)", "lang": "en"}], "type": "LCIA method data set", "refObjectId": "b2ad6494-c78d-11e6-9d9d-cec0c932ce01", "uri": "../lciamethods/b2ad6494-c78d-11e6-9d9d-cec0c932ce01.xml"}, "other": {"anies": [{"name": "referenceToUnitGroupDataSet", "value": {"shortDescription": [{"value": "kg Sb-Äq.", "lang": "de"}], "type": "unit group data set", "refObjectId": "54ccd2d9-a32a-4fc2-923d-f2c8c93e89d4", "uri": "../unitgroups/54ccd2d9-a32a-4fc2-923d-f2c8c93e89d4.xml"}}, {"value": "0.106797386102669", "module": "A1-A3"}, {"value": "0", "module": "C1"}, {"value": "2.65013565513285E-07", "module": "C2"}, {"value": "0", "module": "C3"}, {"value": "1.68496269109713E-07", "module": "C4"}, {"value": "-0.00503343075715077", "module": "D"}]}}, {"referenceToLCIAMethodDataSet": {"shortDescription": [{"value": "Potenzial für den abiotischen Abbau fossiler Brennstoffe (ADPF)", "lang": "de"}, {"value": "Abiotic depletion potential for fossil resources (ADPF)", "lang": "en"}], "type": "LCIA method data set", "refObjectId": "b2ad6110-c78d-11e6-9d9d-cec0c932ce01", "uri": "../lciamethods/b2ad6110-c78d-11e6-9d9d-cec0c932ce01.xml"}, "other": {"anies": [{"name": "referenceToUnitGroupDataSet", "value": {"shortDescription": [{"value": "MJ", "lang": "de"}], "type": "unit group data set", "refObjectId": "93a60a57-a3c8-11da-a746-0800200c9a66", "uri": "../unitgroups/93a60a57-a3c8-11da-a746-0800200c9a66.xml"}}, {"value": "48745.0275883345", "module": "A1-A3"}, {"value": "0", "module": "C1"}, {"value": "39.8249241581825", "module": "C2"}, {"value": "0", "module": "C3"}, {"value": "35.5528764029718", "module": "C4"}, {"value": "-20135.11896145", "module": "D"}]}}, {"referenceToLCIAMethodDataSet": {"shortDescription": [{"value": "Wassernutzung (WDP)", "lang": "de"}, {"value": "Water use (WDP)", "lang": "en"}], "type": "LCIA method data set", "refObjectId": "b2ad66ce-c78d-11e6-9d9d-cec0c932ce01", "uri": "../lciamethods/b2ad66ce-c78d-11e6-9d9d-cec0c932ce01.xml"}, "other": {"anies": [{"name": "referenceToUnitGroupDataSet", "value": {"shortDescription": [{"value": "m^(3) Welt-Äq. entzogen", "lang": "de"}], "type": "unit group data set", "refObjectId": "6ae2df01-888e-46c8-b17d-49fa3869b476", "uri": "../unitgroups/6ae2df01-888e-46c8-b17d-49fa3869b476.xml"}}, {"value": "226.718449413605", "module": "A1-A3"}, {"value": "0", "module": "C1"}, {"value": "0.0277457256015725", "module": "C2"}, {"value": "0", "module": "C3"}, {"value": "-0.0289389620167935", "module": "C4"}, {"value": "-453.948845109142", "module": "D"}]}}, {"referenceToLCIAMethodDataSet": {"shortDescription": [{"value": "Auftreten von Krankheiten aufgrund von Feinstaubemissionen (PM)", "lang": "de"}, {"value": "Incidence of disease due to PM emissions (PM)", "lang": "en"}], "type": "LCIA method data set", "refObjectId": "b5c602c6-def3-11e6-bf01-fe55135034f3", "uri": "../lciamethods/b5c602c6-def3-11e6-bf01-fe55135034f3.xml"}, "other": {"anies": [{"name": "referenceToUnitGroupDataSet", "value": {"shortDescription": [{"value": "Krankheitsfälle", "lang": "de"}], "type": "unit group data set", "refObjectId": "3883559b-648f-4afc-8ba2-0bd24f3affa3", "uri": "../unitgroups/3883559b-648f-4afc-8ba2-0bd24f3affa3.xml"}}, {"module": "A1-A3"}, {"module": "C1"}, {"module": "C2"}, {"module": "C3"}, {"module": "C4"}, {"module": "D"}]}}, {"referenceToLCIAMethodDataSet": {"shortDescription": [{"value": "Wirkung durch Exposition des Menschen mit U235 (IR)", "lang": "de"}, {"value": "Human exposure efficiency relative to U235 (IR)", "lang": "en"}], "type": "LCIA method data set", "refObjectId": "b5c632be-def3-11e6-bf01-fe55135034f3", "uri": "../lciamethods/b5c632be-def3-11e6-bf01-fe55135034f3.xml"}, "other": {"anies": [{"name": "referenceToUnitGroupDataSet", "value": {"shortDescription": [{"value": "kBq U235-Äq.", "lang": "de"}], "type": "unit group data set", "refObjectId": "456b05bf-1415-44a9-9993-02452f554c09", "uri": "../unitgroups/456b05bf-1415-44a9-9993-02452f554c09.xml"}}, {"module": "A1-A3"}, {"module": "C1"}, {"module": "C2"}, {"module": "C3"}, {"module": "C4"}, {"module": "D"}]}}, {"referenceToLCIAMethodDataSet": {"shortDescription": [{"value": "Toxizitätsvergleichseinheit für Ökosysteme (ETP-fw)", "lang": "de"}, {"value": "Comparative toxic unit for ecosystems (ETP-fw)", "lang": "en"}], "type": "LCIA method data set", "refObjectId": "ee1082d1-b0f7-43ca-a1f0-21e2a4a74511", "uri": "../lciamethods/ee1082d1-b0f7-43ca-a1f0-21e2a4a74511.xml"}, "other": {"anies": [{"name": "referenceToUnitGroupDataSet", "value": {"shortDescription": [{"value": "CTUe", "lang": "de"}], "type": "unit group data set", "refObjectId": "aa959ded-f1eb-4efb-9c5c-2d60be36b3e6", "uri": "../unitgroups/aa959ded-f1eb-4efb-9c5c-2d60be36b3e6.xml"}}, {"module": "A1-A3"}, {"module": "C1"}, {"module": "C2"}, {"module": "C3"}, {"module": "C4"}, {"module": "D"}]}}, {"referenceToLCIAMethodDataSet": {"shortDescription": [{"value": "Toxizitätsvergleichseinheit für Menschen (krebserregend) (HTP-c)", "lang": "de"}, {"value": "Comparative toxic unit for humans (carcinogenic) (HTP-c)", "lang": "en"}], "type": "LCIA method data set", "refObjectId": "2299222a-bbd8-474f-9d4f-4dd1f18aea7c", "uri": "../lciamethods/2299222a-bbd8-474f-9d4f-4dd1f18aea7c.xml"}, "other": {"anies": [{"name": "referenceToUnitGroupDataSet", "value": {"shortDescription": [{"value": "CTUh", "lang": "de"}], "type": "unit group data set", "refObjectId": "d4c9523e-2d7e-49fd-8469-998f547d3a70", "uri": "../unitgroups/d4c9523e-2d7e-49fd-8469-998f547d3a70.xml"}}, {"module": "A1-A3"}, {"module": "C1"}, {"module": "C2"}, {"module": "C3"}, {"module": "C4"}, {"module": "D"}]}}, {"referenceToLCIAMethodDataSet": {"shortDescription": [{"value": "Toxizitätsvergleichseinheit für Menschen (nicht krebserregend) (HTP-nc)", "lang": "de"}, {"value": "Comparative toxic unit for humans (noncarcinogenic) (HTP-nc)", "lang": "en"}], "type": "LCIA method data set", "refObjectId": "3af763a5-b7a1-48c9-9cee-1f223481fcef", "uri": "../lciamethods/3af763a5-b7a1-48c9-9cee-1f223481fcef.xml"}, "other": {"anies": [{"name": "referenceToUnitGroupDataSet", "value": {"shortDescription": [{"value": "CTUh", "lang": "de"}], "type": "unit group data set", "refObjectId": "d4c9523e-2d7e-49fd-8469-998f547d3a70", "uri": "../unitgroups/d4c9523e-2d7e-49fd-8469-998f547d3a70.xml"}}, {"module": "A1-A3"}, {"module": "C1"}, {"module": "C2"}, {"module": "C3"}, {"module": "C4"}, {"module": "D"}]}}, {"referenceToLCIAMethodDataSet": {"shortDescription": [{"value": "Bodenqualitätsindex (SQP)", "lang": "de"}, {"value": "Soil quality index (SQP)", "lang": "en"}], "type": "LCIA method data set", "refObjectId": "b2ad6890-c78d-11e6-9d9d-cec0c932ce01", "uri": "../lciamethods/b2ad6890-c78d-11e6-9d9d-cec0c932ce01.xml"}, "other": {"anies": [{"name": "referenceToUnitGroupDataSet", "value": {"shortDescription": [{"value": "SQP", "lang": "de"}], "type": "unit group data set", "refObjectId": "f130951c-e67f-4f7f-8dd4-665de3974e18", "uri": "../unitgroups/f130951c-e67f-4f7f-8dd4-665de3974e18.xml"}}, {"module": "A1-A3"}, {"module": "C1"}, {"module": "C2"}, {"module": "C3"}, {"module": "C4"}, {"module": "D"}]}}]}, "otherAttributes": {"{http://www.indata.network/EPD/2019}epd-version": "1.2"}, "version": "1.1", "locations": "../ILCDLocations.xml"}