{"processInformation": {"dataSetInformation": {"UUID": "5c536009-b0a8-4539-86c2-c3b8247f7f1a", "name": {"baseName": [{"value": "TILLY Naturholzplatte", "lang": "de"}, {"value": "TILLY solid wood panel", "lang": "en"}], "functionalUnitFlowProperties": [{"lang": "de"}]}, "classificationInformation": {"classification": [{"class": [{"value": "Holz", "level": 0, "classId": "3"}, {"value": "Vollholz", "level": 1, "classId": "3.1"}, {"value": "Brettschichtholzplatte", "level": 2, "classId": "3.1.05"}], "name": "OEKOBAU.DAT"}, {"class": [{"value": "02 Bauprodukte", "level": 0}, {"value": "Produkte aus Bauholz", "level": 1}, {"value": "Vollholzprodukte", "level": 2}], "name": "IBUCategories"}]}, "generalComment": [{"value": "TILLY Dreischicht-Naturholzplatten sind mehrschichtige Massivholzplatten gem. EN 13353, bei denen zwei zueinander parallellaufende Deckschichten mit einer um 90° versetzten Mittellage (Absperreffekt) verleimt sind. Die Stabmittellagen sind in der Lnge keilgezinkt. Die Decklagen sind aus fugendicht verleimten durchgehenden Einzellamellen hergestellt. Decklage und Mittellage bestehen grundstzlich aus der gleichen Holzart. Produktionsseitige nderungen vorbehalten. \n\nNeben der Tilly Dreischicht-Massivholzplatte werden auch Einschicht-Massivholzplatten hergestellt. Die Einschicht-Massivholzplatte (auch bekannt als Leimholz-Platte) besteht aus stumpf miteinander verleimten, durchgehenden (nicht keilgezinkten) Holzlatten, deren Oberseite qualittssortiert ist.\n\nAlle produzierten Mehrschichtplatten (Ein-, Zwei- und Dreischichtplatten) inklusive Sonderausfhrungen (Trrohlinge und Trfriesen) sind Teil dieser EPD.", "lang": "de"}, {"value": "TILLY three-layer natural wood panels are multi-layer solid wood panels in accordance with EN 13353, in which two face layers running parallel to each other are glued together with a centre layer offset by 90 degrees (blocking effect). The middle layers are finger-jointed along their length. The top layers are made of joint-tight glued continuous single lamellae. The top layer and middle layer are always made of the same type of wood. Subject to changes on the production side. \n\nIn addition to the Tilly three-layer solid wood panel, single-layer solid wood panels are also produced. The single-layer solid wood panel consists of continuous (not finger-jointed) wood strips glued together butt-jointed, the top side of which is quality-graded. \n\nAll multi-layer boards produced (single-, two- and three-layer boards) including special designs (door blanks and doorframes) are part of this EPD.", "lang": "en"}]}, "quantitativeReference": {"referenceToReferenceFlow": [0]}, "time": {"referenceYear": 2023, "dataSetValidUntil": 2028, "other": {"anies": [{"name": "publicationDateOfEPD", "value": 1687305600000}]}}, "geography": {"locationOfOperationSupplyOrProduction": {"location": "AT"}}, "technology": {"technologyDescriptionAndIncludedProcesses": [{"value": "Rohstoffbeschaffung und Vorproduktion: Das eingesetzte Holz wird aus Mitteleuropa mit Nachhaltigkeitszertifikat (PEFC-CoC zertifiziert) zugekauft. Das Schnittholz wird technisch bei Temperaturen bis zu 90°C auf eine Endfeuchte von u=8 % getrocknet. Mehrschichtige Massivholzplatten bestehen aus drei um jeweils 90° versetzt flächenförmig miteinander verleimten Lamellenschichten (Decklagen und Mittellage).  Decklamellen: Die getrockneten Bretter werden mittels Bandsägen in Lamellen aufgetrennt und anschließend einer maschinellen Qualitätssortierung unterzogen und in die Erscheinungsklassen 0, A, B und C, analog EN 13017-1 Nadelholz bzw. EN 13017-2 Laubholz sortiert. Mittellage: Die Vorfertigung der keilgezinkten Stabmittellagen erfolgt in einer Durchlaufpresse. Dabei werden die Lamellenschmalflächen mit einer PVAc-Dispersion beleimt und mit Hochfrequenzaushärtung zu Mittellagen-Teppichen verpresst (Transportverleimung). Verpressung: Zur Herstellung der dreilagigen Platten wird die vorgefertigte Mittellage breitflächig und beidseitig mittels Walzenauftragsmaschine mit dem heißaushärtenden MUF-Harz-System zzgl. Härter beleimt. Die Lamellen der Decklagen werden zusätzlich unter Druck fugenverleimt. Nach der Verpressung in Mehretagen-Presse mit zusätzlichem Seitendruck bei einer Presstemperatur von bis zu 115 °C, konditionieren die Platten mindestens 24 h im Stapel und werden dabei wieder abgekühlt.  Einschichtige Massivholzplatten bestehen aus durchgehenden (nicht keilgezinkten), qualitätssortierten Holzlatten, die mit einem kaltaushärtenden PU-Klebstoff stumpf an den Schmalseiten in einer Durchlaufpresse miteinander verleimt werden.  Endfertigung: Anschließend erfolgt für alle Platten eine Fehlstellenausbesserung (Äste, Harzgallen) nach definierten Richtlinien, dann die Längs- und Querformatierung und der Kalibrierschliff mit Korn 60 und 100 auf die jeweilige Nenndicke. Die Produktion erfolgt nach den Normen EN 13986, EN 13017-1, EN 13353. Die Qualitätskontrolle ist produktionsbegleitend durch ein Qualitätsmanagementsystem nach ISO 9001 geregelt. Es kommen keinerlei chemische Holzschutzmittel zum Einsatz. \nTechnische Daten: \nDie dicke- und produktabhngigen Leistungsdaten entsprechen der jeweils \nproduktzugehrigen Leistungserklrung in der letztgltigen Fassung. Die Leistungserklrungen sind online auf www.tilly.at unter Service/Leistungserklrung in der jeweiligen Landessprache zu finden. ltere Versionen der Leistungserklrungen knnen unter office.platten@tilly.at angefordert werden. Folgende bautechnische Daten gelten nur fr Dreischicht-Naturholzplatten 17–60 mm: \nDeklarierte Einheit: \nDie vorliegende Umwelt-Produktdeklaration bezieht sich auf eine deklarierte Einheit von 1 m TILLY Massivholzplatte mit einer durchschnittlichen Dichte von 473 kg/m.", "lang": "de"}, {"value": "Procurement of raw materials and preliminary production: The wood used is purchased in central Europe with a sustainability certificate (PEFC-CoC-certified). The sawn timber is technically dried at temperatures up to 90 °C to a final moisture content of u = 8%. Multi-layer solid wood panels consist of three lamella layers (facing top layers and core layer) glued together, each offset by 90°. Top lamellas: The dried boards are cut into lamellas by band saws and then subjected to machine-quality grading and sorted into appearance classes 0, A, B and C, analogous to EN 13017-1 Softwood or EN 13017-2 Hardwood. Core layer: Prefabrication of the finger-jointed bar core layers is carried out in a continuous press. The narrow lamella surfaces are glued with a PVAc dispersion and pressed into core layer carpets with high-frequency curing (transport gluing). Pressing: To produce the three-layer panels, the prefabricated core layer is glued over a wide area and on both sides by means of a roller applicator with the heat-curing MUF resin system plus hardener. The lamellas of the top layers are additionally joint-glued under pressure. After pressing in a multi-layer press with additional side pressure at a press temperature of up to 115 °C, the boards are conditioned in the stack for at least 24 hours and are cooled down again in the process. Single-layer solid wood panels consist of continuous (not finger-jointed), quality-sorted wooden slats, which are glued together butt-jointed on the narrow sides in a continuous press using a cold-curing PU adhesive. Finishing: Subsequently, all boards are defect-repaired (knots, resin pockets) according to defined guidelines, then formatted lengthwise and crosswise and calibration-sanded with grit 60 and 100 to the respective nominal thickness. Production is in accordance with the EN 13986, EN 13017-1 and EN 13353 standards. Quality control during production is regulated by a quality management system according to ISO 9001. No chemical wood preservatives are used. \nTechnical data: \nThe thickness- and product-dependent performance data corresponds to the respective product-related Declaration of Performance in its latest valid version. The Declarations of Performance can be found online at www.tilly.at under Service/Declaration of Performance in the respective national language. Older versions of the Declarations of Performance can be requested from office.platten@tilly.at. The following structural data only applies to three-layer natural wood panels 17-60 mm: \nDeclared unit: \nThis EPD refers to a declared unit of 1 m of TILLY solid wood panels with an average density of 473 kg/m.", "lang": "en"}], "technologicalApplicability": [{"value": "Tilly Naturholzplatten finden neben der optischen Anwendung im Mbelbau, tragenden und nicht tragenden Innenausbau (Boden, Wand, Decke) auch Verwendung als tragende und aussteifende Beplankung im Trocken-, Feucht- oder im geschtzten Auenbereich.", "lang": "de"}, {"value": "Tilly natural wood panels are used not only for visual applications in furniture construction, load-bearing and non-load-bearing interior fittings (floors, walls, ceilings), but also as load-bearing and stiffening planking in dry, wet or protected outdoor areas.", "lang": "en"}]}}, "modellingAndValidation": {"LCIMethodAndAllocation": {"typeOfDataSet": "EPD", "referenceToLCAMethodDetails": [{"shortDescription": [{"value": "Vollholzprodukte.pdf", "lang": "de"}], "type": "source data set", "refObjectId": "74ba5045-d4a3-42ec-aa2a-9273345009c6"}], "other": {"anies": [{"name": "subType", "value": "average dataset"}]}}, "dataSourcesTreatmentAndRepresentativeness": {"referenceToDataSource": [{"shortDescription": [{"value": "GaBi Database (all versions)", "lang": "de"}], "type": "source data set", "refObjectId": "28d74cc0-db8b-4d7e-bc44-5f6d56ce0c4a"}, {"shortDescription": [{"value": "GaBi Database Edition 2022, CUP 2022.02", "lang": "de"}], "type": "source data set", "refObjectId": "94f442cb-662e-43ea-a792-4b0a35132e93"}], "useAdviceForDataSet": [{"value": "Gültigkeitsbereich: \nDieses Dokument bezieht sich auf 1 m TILLY Naturholzplatte, produziert in Althofen, sterreich.\nDarin wurden TILLY Ein-, Zwei- und Dreischichtplatten sowie die Produktion von Sonderprodukten (Trrohlinge & Trfriesen) bercksichtigt. \nSystemgrenze: \nDie kobilanz der TILLY Massivholzplatten beinhaltet eine cradle-to-gate with options (Wiege bis zum Werkstor mit Optionen)-Betrachtung der auftretenden Umweltwirkungen mit den Modulen C1–C4 und Modul D (A1–A3, + C, + D). Die folgenden Lebenszyklusphasen werden in der Analyse bercksichtigt:\n\nModul A1–A3 | Produktionsstadium\nDas Produktionsstadium beinhaltet die Aufwendungen der Rohstoffversorgung (Schnittholz, Herstellung des Leimsystems etc.) sowie der damit verbundenen Transporte bezogen auf den Produktionsstandort in Althofen. Innerhalb der Werksgrenzen werden die Holztrocknung, das Auftrennen des Schnittholzes, die visuelle Sortierung, das Verpressen der Platten, die Schleifanlage sowie der Plattenzuschnitt inklusive der Verpackung des Produkts bercksichtigt. Der Standort Althofen bezieht 100 % kostrom. Zustzlich wird am Standort elektrische Energie ber eine Photovoltaik-Anlage, ein Wasserkraftwerk sowie eine werkseigene Biomasseanlage erzeugt. Die Wrmebereitstellung am Standort erfolgt ber die Biomasseanlage. \n\nModul C1 | Rckbau/Abriss\nFr die Massivholzplatten wurde ein manueller Ausbau angenommen. Die damit verbundenen Aufwnde sind vernachlssigbar, wodurch keine Umweltwirkungen aus dem Rckbau der Produkte deklariert werden.\n\nModul C2 | Transport zur Abfallbehandlung\nModul C2 beinhaltet den Transport zur Abfallbehandlung. Dazu wird der Transport via LKW ber 50 km Transportdistanz als reprsentatives Szenario angesetzt.\n\nModul C3 | Abfallbehandlung \nIn Modul C3 wird das Hacken nach Ausbau der Produkte betrachtet. Die Holzprodukte und mit ihnen die materialinhrenten Eigenschaften verlassen das Produktsystem als Sekundrbrennstoff in Modul C3. \nIn der energetischen Verwertung am Lebensende des Produktes wird biogener Kohlenstoff, der im Produkt gebunden ist, frei. Die damit verbundene, biogene Kohlendioxid-Emission wird in Modul C3 bilanziert. Damit ist die Kohlenstoffbilanz innerhalb der Systemgrenze des Produktsystems geschlossen. \n\nModul C4 | Beseitigung\nDas angesetzte Szenario deklariert die energetische Verwertung der Holzprodukte, wodurch keine Umweltauswirkungen aus der Abfallbehandlung der Produkte in C4 zu erwarten sind. \n\nModul D | Nutzen und Lasten auerhalb der Systemgrenze \nIn Modul D wird die energetische Verwertung des Produktes am Lebensende inklusive der entstehenden Emissionen (ausgenommen biogener Kohlenstoff deklariert in C3) sowie der entsprechenden energetischen Substitutionspotenziale in Form eines europischen Durchschnittsszenarios beschrieben.", "lang": "de"}, {"value": "Scope: \nThis EPD is based on a declared unit of 1 m of TILLY solid wood panel, produced in Althofen, Austria. The results refer to TILLY single-layer, two-layer and three-layer solid wood panels as well as the production of special products (door blanks & door frames). \nSystem boundary: \nThe life cycle assessment of average TILLY solid wood panels refers to a cradle-to-gate analysis of the environmental impacts with modules C1–C4 and module D (A1–A3 + C + D). The following life cycle phases are part of the analysis:\n\nModule A1–A3 | Production stage\nThe production stage includes upstream burdens of raw materials (sawn timber, adhesive system, etc.) and the corresponding transports to the TILLY production site in Althofen (Austria). Drying, ripping of sawn timber, visual sorting, pressing of the boards, the grinding plant as well as the board cutting including the packaging of the product are taken into account. Althofen is supplied with 100 % green electricity. In addition, electrical energy is generated at the site via a photovoltaic system, a hydroelectric power plant and an in-house biomass plant. Thermal energy is provided at the site via the biomass plant.\n\nModule C1 | Deconstruction and demolition\nManual removal was assumed for the solid wood panels. Associated impacts are negligible, therefore no environmental impacts from the deconstruction of the products are declared.\n\nModule C2 | Transport to disposal\nModule C2 includes the transport to waste treatment. In this case, transport by truck over a transport distance of 50 km is assumed.\n\nModule C3 | Waste processing\nIn Module C3, the chipping after the removal of the products is considered. The wooden products and with them the material-inherent properties leave the product system as secondary \ncombustibles in module C3.\nDuring energy recovery at the products end-of-life, biogenic carbon bound in the product is released. The associated biogenic carbon dioxide emissions are accounted for in Module C3. Thus, the carbon balance within the system boundary of the product system is closed.\n\nModule C4 | Disposal\nThe applied scenario declares the energetic recovery of the wooden products; therefore, no environmental impacts are to be expected from waste processing of the products in C4.\n\nModule D | Benefits and loads beyond the system boundary\nApplying an European average scenario, module D describes the energetic recovery of the product at the end-of-life including the associated emissions (except biogenic carbon declared in C3) as well as corresponding energy substitution potentials.", "lang": "en"}], "other": {"anies": [{"name": "referenceToOriginalEPD", "value": {"shortDescription": {"value": "TILLY Naturholzplatte.pdf", "defaultValue": "TILLY Naturholzplatte.pdf", "lstrings": [{"lang": "de", "value": "TILLY Naturholzplatte.pdf"}]}, "type": "source data set", "uuid": {"uuid": "0ce5daee-57af-4b5a-af88-849a34562109"}, "refObjectId": "0ce5daee-57af-4b5a-af88-849a34562109", "resourceURLs": ["https://oekobaudat.de/OEKOBAU.DAT/resource/sources/0ce5daee-57af-4b5a-af88-849a34562109/TILLY_Naturholzplatte_18089.pdf?version=00.01.000"]}}]}}, "validation": {"review": [{"referenceToNameOfReviewerAndInstitution": [{"shortDescription": [{"value": "Institut Bauen und Umwelt e. V.", "lang": "de"}], "type": "contact data set", "refObjectId": "d111dbec-b024-4be5-86c5-752d6eb2cf95", "uri": "../contacts/d111dbec-b024-4be5-86c5-752d6eb2cf95.xml"}], "type": "Accredited third party review"}]}, "complianceDeclarations": {"compliance": [{"referenceToComplianceSystem": {"shortDescription": [{"value": "DIN EN 15804+A2", "lang": "de"}], "type": "source data set", "refObjectId": "c0016b33-8cf7-415c-ac6e-deba0d21440d", "uri": "../sources/c0016b33-8cf7-415c-ac6e-deba0d21440d.xml"}}, {"referenceToComplianceSystem": {"shortDescription": [{"value": "ISO 14025", "lang": "de"}], "type": "source data set", "refObjectId": "4f2eb655-6e44-4874-a95a-e28f5442cd4d", "uri": "../sources/4f2eb655-6e44-4874-a95a-e28f5442cd4d.xml"}}]}}, "administrativeInformation": {"commissionerAndGoal": {"referenceToCommissioner": [{"shortDescription": [{"value": "Tilly Holzindustrie Gesellschaft m.b.H", "lang": "de"}], "type": "contact data set", "refObjectId": "992e9a1a-3c4b-42e4-a415-a4b1066f2ffc", "uri": "../contacts/992e9a1a-3c4b-42e4-a415-a4b1066f2ffc.xml"}]}, "dataGenerator": {"referenceToPersonOrEntityGeneratingTheDataSet": [{"shortDescription": [{"value": "Daxner & Merl GmbH", "lang": "de"}], "type": "contact data set", "refObjectId": "ad8ad627-3991-42b7-a7ca-5a3fe0a34c28", "uri": "../contacts/ad8ad627-3991-42b7-a7ca-5a3fe0a34c28.xml"}]}, "dataEntryBy": {"timeStamp": 1687305600000, "referenceToDataSetFormat": [{"shortDescription": [{"value": "ILCD Format", "lang": "de"}], "type": "source data set", "refObjectId": "a97a0155-0234-4b87-b4ce-a45da52f2a40", "uri": "../sources/a97a0155-0234-4b87-b4ce-a45da52f2a40.xml"}, {"shortDescription": [{"value": "EPD-Datenformaterweiterungen v1.2", "lang": "de"}, {"value": "EPD Data Format Extensions v1.2", "lang": "en"}], "type": "source data set", "refObjectId": "a29449fd-aa2f-4de8-b5d7-4b06b43c6fde", "uri": "../sources/a29449fd-aa2f-4de8-b5d7-4b06b43c6fde.xml"}]}, "publicationAndOwnership": {"dataSetVersion": "00.01.000", "referenceToRegistrationAuthority": {"shortDescription": [{"value": "Institut Bauen und Umwelt e. V.", "lang": "de"}], "type": "contact data set", "refObjectId": "d111dbec-b024-4be5-86c5-752d6eb2cf95", "uri": "../contacts/d111dbec-b024-4be5-86c5-752d6eb2cf95.xml"}, "registrationNumber": "EPD-TIL-20230209-IBC2-DE", "referenceToOwnershipOfDataSet": {"shortDescription": [{"value": "Tilly Holzindustrie Gesellschaft m.b.H", "lang": "de"}], "type": "contact data set", "refObjectId": "992e9a1a-3c4b-42e4-a415-a4b1066f2ffc", "uri": "../contacts/992e9a1a-3c4b-42e4-a415-a4b1066f2ffc.xml"}, "copyright": true, "licenseType": "Free of charge for all users and uses", "accessRestrictions": [{"value": "None", "lang": "en"}], "other": {"anies": [{"name": "referenceToPublisher", "value": {"shortDescription": [{"value": "Institut Bauen und Umwelt e. V.", "lang": "de"}], "type": "contact data set", "refObjectId": "d111dbec-b024-4be5-86c5-752d6eb2cf95", "uri": "../contacts/d111dbec-b024-4be5-86c5-752d6eb2cf95.xml"}}]}}}, "exchanges": {"exchange": [{"dataSetInternalID": 0, "referenceToFlowDataSet": {"shortDescription": [{"value": "TILLY Massivholzplatte (473 kg/m³) ()", "lang": "de"}], "type": "flow data set", "refObjectId": "a8abf802-b715-0e3e-ccc3-3109190e0c5d", "uri": "../flows/a8abf802-b715-0e3e-ccc3-3109190e0c5d.xml"}, "meanAmount": 1.0, "referencesToDataSource": {}, "referenceFlow": true, "resolvedFlowVersion": "00.01.000", "resultingflowAmount": 1.0, "flowProperties": [{"name": [{"lang": "en", "value": "Volume"}, {"lang": "de", "value": "Volumen"}], "uuid": "93a60a56-a3c8-22da-a746-0800200c9a66", "referenceFlowProperty": true, "meanValue": 1.0, "referenceUnit": "m3", "unitGroupUUID": "cd950537-0a98-4044-9ba7-9f9a68d0a504"}], "materialProperties": [{"name": "gross density", "value": "473.0", "unit": "kg/m^3", "unitDescription": "kilograms per cubic metre"}, {"name": "grammage", "value": "10.4", "unit": "kg/m^2", "unitDescription": "kilograms per square meter"}], "typeOfFlow": "Product flow", "classification": {"classHierarchy": "Holz / Vollholz / Brettschichtholzplatte", "name": "OEKOBAU.DAT"}}, {"dataSetInternalID": 1, "referenceToFlowDataSet": {"shortDescription": [{"value": "Erneuerbare Primärenergie als Energieträger (PERE)", "lang": "de"}, {"value": "Renewable primary energy as energy carrier (PERE)", "lang": "en"}], "type": "flow data set", "refObjectId": "20f32be5-0398-4288-9b6d-accddd195317", "uri": "../flows/20f32be5-0398-4288-9b6d-accddd195317.xml"}, "exchange direction": "INPUT", "other": {"anies": [{"name": "referenceToUnitGroupDataSet", "value": {"shortDescription": [{"value": "MJ", "lang": "de"}], "type": "unit group data set", "refObjectId": "93a60a57-a3c8-11da-a746-0800200c9a66", "uri": "../unitgroups/93a60a57-a3c8-11da-a746-0800200c9a66.xml"}}, {"value": "2459.87606922951", "module": "A1-A3"}, {"value": "0", "module": "C1"}, {"value": "1.29134584775378", "module": "C2"}, {"value": "7937.74496501588", "module": "C3"}, {"value": "0", "module": "C4"}, {"value": "-2194.37409794185", "module": "D"}]}, "resolvedFlowVersion": "38.00.000", "flowProperties": [], "typeOfFlow": "Other flow", "classification": {"classHierarchy": "Quantities", "name": "GaBiCategories"}}, {"dataSetInternalID": 2, "referenceToFlowDataSet": {"shortDescription": [{"value": "Erneuerbare Primärenergie zur stofflichen Nutzung (PERM)", "lang": "de"}, {"value": "Renewable primary energy resources as material utilization (PERM)", "lang": "en"}], "type": "flow data set", "refObjectId": "fb3ec0de-548d-4508-aea5-00b73bf6f702", "uri": "../flows/fb3ec0de-548d-4508-aea5-00b73bf6f702.xml"}, "exchange direction": "INPUT", "other": {"anies": [{"name": "referenceToUnitGroupDataSet", "value": {"shortDescription": [{"value": "MJ", "lang": "de"}], "type": "unit group data set", "refObjectId": "93a60a57-a3c8-11da-a746-0800200c9a66", "uri": "../unitgroups/93a60a57-a3c8-11da-a746-0800200c9a66.xml"}}, {"value": "7903.73447352799", "module": "A1-A3"}, {"value": "0", "module": "C1"}, {"value": "0", "module": "C2"}, {"value": "-7902.61210833162", "module": "C3"}, {"value": "0", "module": "C4"}, {"value": "0", "module": "D"}]}, "resolvedFlowVersion": "38.00.000", "flowProperties": [], "typeOfFlow": "Other flow", "classification": {"classHierarchy": "Quantities", "name": "GaBiCategories"}}, {"dataSetInternalID": 3, "referenceToFlowDataSet": {"shortDescription": [{"value": "Total erneuerbare Primärenergie (PERT)", "lang": "de"}, {"value": "Total use of renewable primary energy resources (PERT)", "lang": "en"}], "type": "flow data set", "refObjectId": "53f97275-fa8a-4cdd-9024-65936002acd0", "uri": "../flows/53f97275-fa8a-4cdd-9024-65936002acd0.xml"}, "exchange direction": "INPUT", "other": {"anies": [{"name": "referenceToUnitGroupDataSet", "value": {"shortDescription": [{"value": "MJ", "lang": "de"}], "type": "unit group data set", "refObjectId": "93a60a57-a3c8-11da-a746-0800200c9a66", "uri": "../unitgroups/93a60a57-a3c8-11da-a746-0800200c9a66.xml"}}, {"value": "10363.6105427575", "module": "A1-A3"}, {"value": "0", "module": "C1"}, {"value": "1.29134584775378", "module": "C2"}, {"value": "35.1328566842636", "module": "C3"}, {"value": "0", "module": "C4"}, {"value": "-2194.37409794185", "module": "D"}]}, "resolvedFlowVersion": "38.00.000", "flowProperties": [], "typeOfFlow": "Other flow", "classification": {"classHierarchy": "Quantities / Environmental quantities / EPD EN 15804 / LCI indicators", "name": "GaBiCategories"}}, {"dataSetInternalID": 4, "referenceToFlowDataSet": {"shortDescription": [{"value": "Nicht-erneuerbare Primärenergie als Energieträger (PENRE)", "lang": "de"}, {"value": "Non renewable primary energy as energy carrier (PENRE)", "lang": "en"}], "type": "flow data set", "refObjectId": "ac857178-2b45-46ec-892a-a9a4332f0372", "uri": "../flows/ac857178-2b45-46ec-892a-a9a4332f0372.xml"}, "exchange direction": "INPUT", "other": {"anies": [{"name": "referenceToUnitGroupDataSet", "value": {"shortDescription": [{"value": "MJ", "lang": "de"}], "type": "unit group data set", "refObjectId": "93a60a57-a3c8-11da-a746-0800200c9a66", "uri": "../unitgroups/93a60a57-a3c8-11da-a746-0800200c9a66.xml"}}, {"value": "1641.51274544846", "module": "A1-A3"}, {"value": "0", "module": "C1"}, {"value": "18.7053864471295", "module": "C2"}, {"value": "274.346799314189", "module": "C3"}, {"value": "0", "module": "C4"}, {"value": "-6949.60837641197", "module": "D"}]}, "resolvedFlowVersion": "38.00.000", "flowProperties": [], "typeOfFlow": "Other flow", "classification": {"classHierarchy": "Quantities", "name": "GaBiCategories"}}, {"dataSetInternalID": 5, "referenceToFlowDataSet": {"shortDescription": [{"value": "Nicht-erneuerbare Primärenergie zur stofflichen Nutzung (PENRM)", "lang": "de"}, {"value": "Non renewable primary energy as material utilization (PENRM)", "lang": "en"}], "type": "flow data set", "refObjectId": "1421caa0-679d-4bf4-b282-0eb850ccae27", "uri": "../flows/1421caa0-679d-4bf4-b282-0eb850ccae27.xml"}, "exchange direction": "INPUT", "other": {"anies": [{"name": "referenceToUnitGroupDataSet", "value": {"shortDescription": [{"value": "MJ", "lang": "de"}], "type": "unit group data set", "refObjectId": "93a60a57-a3c8-11da-a746-0800200c9a66", "uri": "../unitgroups/93a60a57-a3c8-11da-a746-0800200c9a66.xml"}}, {"value": "241.644354591815", "module": "A1-A3"}, {"value": "0", "module": "C1"}, {"value": "0", "module": "C2"}, {"value": "-211.007368979833", "module": "C3"}, {"value": "0", "module": "C4"}, {"value": "0", "module": "D"}]}, "resolvedFlowVersion": "38.00.000", "flowProperties": [], "typeOfFlow": "Other flow", "classification": {"classHierarchy": "Quantities", "name": "GaBiCategories"}}, {"dataSetInternalID": 6, "referenceToFlowDataSet": {"shortDescription": [{"value": "Total nicht erneuerbare Primärenergie (PENRT)", "lang": "de"}, {"value": "Total use of non renewable primary energy resources (PENRT)", "lang": "en"}], "type": "flow data set", "refObjectId": "06159210-646b-4c8d-8583-da9b3b95a6c1", "uri": "../flows/06159210-646b-4c8d-8583-da9b3b95a6c1.xml"}, "exchange direction": "INPUT", "other": {"anies": [{"name": "referenceToUnitGroupDataSet", "value": {"shortDescription": [{"value": "MJ", "lang": "de"}], "type": "unit group data set", "refObjectId": "93a60a57-a3c8-11da-a746-0800200c9a66", "uri": "../unitgroups/93a60a57-a3c8-11da-a746-0800200c9a66.xml"}}, {"value": "1883.15710004027", "module": "A1-A3"}, {"value": "0", "module": "C1"}, {"value": "18.7053864471295", "module": "C2"}, {"value": "63.3394303343564", "module": "C3"}, {"value": "0", "module": "C4"}, {"value": "-6949.60837641197", "module": "D"}]}, "resolvedFlowVersion": "38.00.000", "flowProperties": [], "typeOfFlow": "Other flow", "classification": {"classHierarchy": "Quantities / Environmental quantities / EPD EN 15804 / LCI indicators", "name": "GaBiCategories"}}, {"dataSetInternalID": 7, "referenceToFlowDataSet": {"shortDescription": [{"value": "Einsatz von Sekundärstoffen (SM)", "lang": "de"}, {"value": "Use of secondary material (SM)", "lang": "en"}], "type": "flow data set", "refObjectId": "c6a1f35f-2d09-4f54-8dfb-97e502e1ce92", "uri": "../flows/c6a1f35f-2d09-4f54-8dfb-97e502e1ce92.xml"}, "exchange direction": "INPUT", "other": {"anies": [{"name": "referenceToUnitGroupDataSet", "value": {"shortDescription": [{"value": "kg", "lang": "de"}], "type": "unit group data set", "refObjectId": "ad38d542-3fe9-439d-9b95-2f5f7752acaf", "uri": "../unitgroups/ad38d542-3fe9-439d-9b95-2f5f7752acaf.xml"}}, {"value": "0.00898561167843498", "module": "A1-A3"}, {"value": "0", "module": "C1"}, {"value": "0", "module": "C2"}, {"value": "0", "module": "C3"}, {"value": "0", "module": "C4"}, {"value": "0", "module": "D"}]}, "resolvedFlowVersion": "38.00.000", "flowProperties": [], "typeOfFlow": "Other flow", "classification": {"classHierarchy": "Quantities / Environmental quantities / EPD EN 15804 / LCI indicators", "name": "GaBiCategories"}}, {"dataSetInternalID": 8, "referenceToFlowDataSet": {"shortDescription": [{"value": "Erneuerbare Sekundärbrennstoffe (RSF)", "lang": "de"}, {"value": "Use of renewable secondary fuels (RSF)", "lang": "en"}], "type": "flow data set", "refObjectId": "64333088-a55f-4aa2-9a31-c10b07816787", "uri": "../flows/64333088-a55f-4aa2-9a31-c10b07816787.xml"}, "exchange direction": "INPUT", "other": {"anies": [{"name": "referenceToUnitGroupDataSet", "value": {"shortDescription": [{"value": "MJ", "lang": "de"}], "type": "unit group data set", "refObjectId": "93a60a57-a3c8-11da-a746-0800200c9a66", "uri": "../unitgroups/93a60a57-a3c8-11da-a746-0800200c9a66.xml"}}, {"value": "0", "module": "A1-A3"}, {"value": "0", "module": "C1"}, {"value": "0", "module": "C2"}, {"value": "0", "module": "C3"}, {"value": "0", "module": "C4"}, {"value": "7902.61210833162", "module": "D"}]}, "resolvedFlowVersion": "38.00.000", "flowProperties": [], "typeOfFlow": "Other flow", "classification": {"classHierarchy": "Quantities / Environmental quantities / EPD EN 15804 / LCI indicators", "name": "GaBiCategories"}}, {"dataSetInternalID": 9, "referenceToFlowDataSet": {"shortDescription": [{"value": "Nicht erneuerbare Sekundärbrennstoffe (NRSF)", "lang": "de"}, {"value": "Use of non renewable secondary fuels (NRSF)", "lang": "en"}], "type": "flow data set", "refObjectId": "89def144-d39a-4287-b86f-efde453ddcb2", "uri": "../flows/89def144-d39a-4287-b86f-efde453ddcb2.xml"}, "exchange direction": "INPUT", "other": {"anies": [{"name": "referenceToUnitGroupDataSet", "value": {"shortDescription": [{"value": "MJ", "lang": "de"}], "type": "unit group data set", "refObjectId": "93a60a57-a3c8-11da-a746-0800200c9a66", "uri": "../unitgroups/93a60a57-a3c8-11da-a746-0800200c9a66.xml"}}, {"value": "0", "module": "A1-A3"}, {"value": "0", "module": "C1"}, {"value": "0", "module": "C2"}, {"value": "0", "module": "C3"}, {"value": "0", "module": "C4"}, {"value": "211.007368979833", "module": "D"}]}, "resolvedFlowVersion": "38.00.000", "flowProperties": [], "typeOfFlow": "Other flow", "classification": {"classHierarchy": "Quantities / Environmental quantities / EPD EN 15804 / LCI indicators", "name": "GaBiCategories"}}, {"dataSetInternalID": 10, "referenceToFlowDataSet": {"shortDescription": [{"value": "Einsatz von Süßwasserressourcen (FW)", "lang": "de"}, {"value": "Use of net fresh water (FW)", "lang": "en"}], "type": "flow data set", "refObjectId": "3cf952c8-f3a4-461d-8c96-96456ca62246", "uri": "../flows/3cf952c8-f3a4-461d-8c96-96456ca62246.xml"}, "exchange direction": "INPUT", "other": {"anies": [{"name": "referenceToUnitGroupDataSet", "value": {"shortDescription": [{"value": "m^3", "lang": "de"}], "type": "unit group data set", "refObjectId": "cd950537-0a98-4044-9ba7-9f9a68d0a504", "uri": "../unitgroups/cd950537-0a98-4044-9ba7-9f9a68d0a504.xml"}}, {"value": "1.09695710313508", "module": "A1-A3"}, {"value": "0", "module": "C1"}, {"value": "0.00149173534230858", "module": "C2"}, {"value": "0.0335148497797597", "module": "C3"}, {"value": "0", "module": "C4"}, {"value": "-1.45971853250876", "module": "D"}]}, "resolvedFlowVersion": "38.00.000", "flowProperties": [], "typeOfFlow": "Other flow", "classification": {"classHierarchy": "Quantities / Environmental quantities / EPD EN 15804 / LCI indicators", "name": "GaBiCategories"}}, {"dataSetInternalID": 11, "referenceToFlowDataSet": {"shortDescription": [{"value": "Gefährlicher Abfall zur Deponie (HWD)", "lang": "de"}, {"value": "Hazardous waste disposed (HWD)", "lang": "en"}], "type": "flow data set", "refObjectId": "430f9e0f-59b2-46a0-8e0d-55e0e84948fc", "uri": "../flows/430f9e0f-59b2-46a0-8e0d-55e0e84948fc.xml"}, "exchange direction": "OUTPUT", "other": {"anies": [{"name": "referenceToUnitGroupDataSet", "value": {"shortDescription": [{"value": "kg", "lang": "de"}], "type": "unit group data set", "refObjectId": "ad38d542-3fe9-439d-9b95-2f5f7752acaf", "uri": "../unitgroups/ad38d542-3fe9-439d-9b95-2f5f7752acaf.xml"}}, {"value": "3.26795910136915E-07", "module": "A1-A3"}, {"value": "0", "module": "C1"}, {"value": "9.89739768863647E-11", "module": "C2"}, {"value": "5.47727987511154E-09", "module": "C3"}, {"value": "0", "module": "C4"}, {"value": "-4.27647440580992E-07", "module": "D"}]}, "resolvedFlowVersion": "38.00.000", "flowProperties": [], "typeOfFlow": "Other flow", "classification": {"classHierarchy": "Quantities / Environmental quantities / EPD EN 15804 / LCI indicators", "name": "GaBiCategories"}}, {"dataSetInternalID": 12, "referenceToFlowDataSet": {"shortDescription": [{"value": "Entsorgter nicht gefährlicher Abfall (NHWD)", "lang": "de"}, {"value": "Non hazardous waste disposed (NHWD)", "lang": "en"}], "type": "flow data set", "refObjectId": "b29ef66b-e286-4afa-949f-62f1a7b4d7fa", "uri": "../flows/b29ef66b-e286-4afa-949f-62f1a7b4d7fa.xml"}, "exchange direction": "OUTPUT", "other": {"anies": [{"name": "referenceToUnitGroupDataSet", "value": {"shortDescription": [{"value": "kg", "lang": "de"}], "type": "unit group data set", "refObjectId": "ad38d542-3fe9-439d-9b95-2f5f7752acaf", "uri": "../unitgroups/ad38d542-3fe9-439d-9b95-2f5f7752acaf.xml"}}, {"value": "2.5686459658886", "module": "A1-A3"}, {"value": "0", "module": "C1"}, {"value": "0.00304757293477083", "module": "C2"}, {"value": "0.0476851464854865", "module": "C3"}, {"value": "0", "module": "C4"}, {"value": "0.169017601581418", "module": "D"}]}, "resolvedFlowVersion": "38.00.000", "flowProperties": [], "typeOfFlow": "Other flow", "classification": {"classHierarchy": "Quantities / Environmental quantities / EPD EN 15804 / LCI indicators", "name": "GaBiCategories"}}, {"dataSetInternalID": 13, "referenceToFlowDataSet": {"shortDescription": [{"value": "Entsorgter radioaktiver Abfall (RWD)", "lang": "de"}, {"value": "Radioactive waste disposed (RWD)", "lang": "en"}], "type": "flow data set", "refObjectId": "3449546e-52ad-4b39-b809-9fb77cea8ff6", "uri": "../flows/3449546e-52ad-4b39-b809-9fb77cea8ff6.xml"}, "exchange direction": "OUTPUT", "other": {"anies": [{"name": "referenceToUnitGroupDataSet", "value": {"shortDescription": [{"value": "kg", "lang": "de"}], "type": "unit group data set", "refObjectId": "ad38d542-3fe9-439d-9b95-2f5f7752acaf", "uri": "../unitgroups/ad38d542-3fe9-439d-9b95-2f5f7752acaf.xml"}}, {"value": "0.0254406062179198", "module": "A1-A3"}, {"value": "0", "module": "C1"}, {"value": "3.4722588642336E-05", "module": "C2"}, {"value": "0.0101165508678383", "module": "C3"}, {"value": "0", "module": "C4"}, {"value": "-0.630104134387593", "module": "D"}]}, "resolvedFlowVersion": "38.00.000", "flowProperties": [], "typeOfFlow": "Other flow", "classification": {"classHierarchy": "Quantities / Environmental quantities / EPD EN 15804 / LCI indicators", "name": "GaBiCategories"}}, {"dataSetInternalID": 14, "referenceToFlowDataSet": {"shortDescription": [{"value": "Komponenten für die Wiederverwendung (CRU)", "lang": "de"}, {"value": "Components for re-use (CRU)", "lang": "en"}], "type": "flow data set", "refObjectId": "a2b32f97-3fc7-4af2-b209-525bc6426f33", "uri": "../flows/a2b32f97-3fc7-4af2-b209-525bc6426f33.xml"}, "exchange direction": "OUTPUT", "other": {"anies": [{"name": "referenceToUnitGroupDataSet", "value": {"shortDescription": [{"value": "kg", "lang": "de"}], "type": "unit group data set", "refObjectId": "ad38d542-3fe9-439d-9b95-2f5f7752acaf", "uri": "../unitgroups/ad38d542-3fe9-439d-9b95-2f5f7752acaf.xml"}}, {"value": "0", "module": "A1-A3"}, {"value": "0", "module": "C1"}, {"value": "0", "module": "C2"}, {"value": "0", "module": "C3"}, {"value": "0", "module": "C4"}, {"value": "0", "module": "D"}]}, "resolvedFlowVersion": "38.00.000", "flowProperties": [], "typeOfFlow": "Other flow", "classification": {"classHierarchy": "Quantities / Environmental quantities / EPD EN 15804 / LCI indicators", "name": "GaBiCategories"}}, {"dataSetInternalID": 15, "referenceToFlowDataSet": {"shortDescription": [{"value": "Stoffe zum Recycling (MFR)", "lang": "de"}, {"value": "Materials for recycling (MFR)", "lang": "en"}], "type": "flow data set", "refObjectId": "d7fe48a5-4103-49c8-9aae-b0b5dfdbd6ae", "uri": "../flows/d7fe48a5-4103-49c8-9aae-b0b5dfdbd6ae.xml"}, "exchange direction": "OUTPUT", "other": {"anies": [{"name": "referenceToUnitGroupDataSet", "value": {"shortDescription": [{"value": "kg", "lang": "de"}], "type": "unit group data set", "refObjectId": "ad38d542-3fe9-439d-9b95-2f5f7752acaf", "uri": "../unitgroups/ad38d542-3fe9-439d-9b95-2f5f7752acaf.xml"}}, {"value": "0", "module": "A1-A3"}, {"value": "0", "module": "C1"}, {"value": "0", "module": "C2"}, {"value": "0", "module": "C3"}, {"value": "0", "module": "C4"}, {"value": "0", "module": "D"}]}, "resolvedFlowVersion": "38.00.000", "flowProperties": [], "typeOfFlow": "Other flow", "classification": {"classHierarchy": "Quantities / Environmental quantities / EPD EN 15804 / LCI indicators", "name": "GaBiCategories"}}, {"dataSetInternalID": 16, "referenceToFlowDataSet": {"shortDescription": [{"value": "Stoffe für die Energierückgewinnung (MER)", "lang": "de"}, {"value": "Materials for energy recovery (MER)", "lang": "en"}], "type": "flow data set", "refObjectId": "59a9181c-3aaf-46ee-8b13-2b3723b6e447", "uri": "../flows/59a9181c-3aaf-46ee-8b13-2b3723b6e447.xml"}, "exchange direction": "OUTPUT", "other": {"anies": [{"name": "referenceToUnitGroupDataSet", "value": {"shortDescription": [{"value": "kg", "lang": "de"}], "type": "unit group data set", "refObjectId": "ad38d542-3fe9-439d-9b95-2f5f7752acaf", "uri": "../unitgroups/ad38d542-3fe9-439d-9b95-2f5f7752acaf.xml"}}, {"value": "0", "module": "A1-A3"}, {"value": "0", "module": "C1"}, {"value": "0", "module": "C2"}, {"value": "472.787895040978", "module": "C3"}, {"value": "0", "module": "C4"}, {"value": "0", "module": "D"}]}, "resolvedFlowVersion": "38.00.000", "flowProperties": [], "typeOfFlow": "Other flow", "classification": {"classHierarchy": "Quantities / Environmental quantities / EPD EN 15804 / LCI indicators", "name": "GaBiCategories"}}, {"dataSetInternalID": 17, "referenceToFlowDataSet": {"shortDescription": [{"value": "Exportierte elektrische Energie (EEE)", "lang": "de"}, {"value": "Exported electrical energy (EEE)", "lang": "en"}], "type": "flow data set", "refObjectId": "4da0c987-2b76-40d6-9e9e-82a017aaaf29", "uri": "../flows/4da0c987-2b76-40d6-9e9e-82a017aaaf29.xml"}, "exchange direction": "OUTPUT", "other": {"anies": [{"name": "referenceToUnitGroupDataSet", "value": {"shortDescription": [{"value": "MJ", "lang": "de"}], "type": "unit group data set", "refObjectId": "93a60a57-a3c8-11da-a746-0800200c9a66", "uri": "../unitgroups/93a60a57-a3c8-11da-a746-0800200c9a66.xml"}}, {"value": "0", "module": "A1-A3"}, {"value": "0", "module": "C1"}, {"value": "0", "module": "C2"}, {"value": "0", "module": "C3"}, {"value": "0", "module": "C4"}, {"value": "0", "module": "D"}]}, "resolvedFlowVersion": "38.00.000", "flowProperties": [], "typeOfFlow": "Other flow", "classification": {"classHierarchy": "Quantities / Environmental quantities / EPD EN 15804 / LCI indicators", "name": "GaBiCategories"}}, {"dataSetInternalID": 18, "referenceToFlowDataSet": {"shortDescription": [{"value": "Exportierte thermische Energie (EET)", "lang": "de"}, {"value": "Exported thermal energy (EET)", "lang": "en"}], "type": "flow data set", "refObjectId": "98daf38a-7a79-46d3-9a37-2b7bd0955810", "uri": "../flows/98daf38a-7a79-46d3-9a37-2b7bd0955810.xml"}, "exchange direction": "OUTPUT", "other": {"anies": [{"name": "referenceToUnitGroupDataSet", "value": {"shortDescription": [{"value": "MJ", "lang": "de"}], "type": "unit group data set", "refObjectId": "93a60a57-a3c8-11da-a746-0800200c9a66", "uri": "../unitgroups/93a60a57-a3c8-11da-a746-0800200c9a66.xml"}}, {"value": "0", "module": "A1-A3"}, {"value": "0", "module": "C1"}, {"value": "0", "module": "C2"}, {"value": "0", "module": "C3"}, {"value": "0", "module": "C4"}, {"value": "0", "module": "D"}]}, "resolvedFlowVersion": "38.00.000", "flowProperties": [], "typeOfFlow": "Other flow", "classification": {"classHierarchy": "Quantities / Environmental quantities / EPD EN 15804 / LCI indicators", "name": "GaBiCategories"}}]}, "LCIAResults": {"LCIAResult": [{"referenceToLCIAMethodDataSet": {"shortDescription": [{"value": "Globales Erwärmungspotenzial total (GWP-total)", "lang": "de"}, {"value": "Global Warming Potential total (GWP-total)", "lang": "en"}], "type": "LCIA method data set", "refObjectId": "6a37f984-a4b3-458a-a20a-64418c145fa2", "uri": "../lciamethods/6a37f984-a4b3-458a-a20a-64418c145fa2.xml"}, "other": {"anies": [{"name": "referenceToUnitGroupDataSet", "value": {"shortDescription": [{"value": "kg CO_(2)-Äq.", "lang": "de"}], "type": "unit group data set", "refObjectId": "1ebf3012-d0db-4de2-aefd-ef30cedb0be1", "uri": "../unitgroups/1ebf3012-d0db-4de2-aefd-ef30cedb0be1.xml"}}, {"value": "-664.253673636496", "module": "A1-A3"}, {"value": "0", "module": "C1"}, {"value": "1.43256924040229", "module": "C2"}, {"value": "786.606315387412", "module": "C3"}, {"value": "0", "module": "C4"}, {"value": "-403.472658564922", "module": "D"}]}}, {"referenceToLCIAMethodDataSet": {"shortDescription": [{"value": "Globales Erwärmungspotenzial fossil (GWP-fossil)", "lang": "de"}, {"value": "Global Warming Potential fossil fuels (GWP-fossil)", "lang": "en"}], "type": "LCIA method data set", "refObjectId": "5f635281-343e-44fb-83df-1971b155e6b6", "uri": "../lciamethods/5f635281-343e-44fb-83df-1971b155e6b6.xml"}, "other": {"anies": [{"name": "referenceToUnitGroupDataSet", "value": {"shortDescription": [{"value": "kg CO_(2)-Äq.", "lang": "de"}], "type": "unit group data set", "refObjectId": "1ebf3012-d0db-4de2-aefd-ef30cedb0be1", "uri": "../unitgroups/1ebf3012-d0db-4de2-aefd-ef30cedb0be1.xml"}}, {"value": "113.582009797812", "module": "A1-A3"}, {"value": "0", "module": "C1"}, {"value": "1.42300514900505", "module": "C2"}, {"value": "3.48852117247826", "module": "C3"}, {"value": "0", "module": "C4"}, {"value": "-401.134359656445", "module": "D"}]}}, {"referenceToLCIAMethodDataSet": {"shortDescription": [{"value": "Globales Erwärmungspotenzial biogen (GWP-biogenic)", "lang": "de"}, {"value": "Global Warming Potential biogenic (GWP-biogenic)", "lang": "en"}], "type": "LCIA method data set", "refObjectId": "2356e1ab-0185-4db5-86e5-16de51c7485c", "uri": "../lciamethods/2356e1ab-0185-4db5-86e5-16de51c7485c.xml"}, "other": {"anies": [{"name": "referenceToUnitGroupDataSet", "value": {"shortDescription": [{"value": "kg CO_(2)-Äq.", "lang": "de"}], "type": "unit group data set", "refObjectId": "1ebf3012-d0db-4de2-aefd-ef30cedb0be1", "uri": "../unitgroups/1ebf3012-d0db-4de2-aefd-ef30cedb0be1.xml"}}, {"value": "-778.132920477231", "module": "A1-A3"}, {"value": "0", "module": "C1"}, {"value": "0", "module": "C2"}, {"value": "783.117056588329", "module": "C3"}, {"value": "0", "module": "C4"}, {"value": "-2.28928687777496", "module": "D"}]}}, {"referenceToLCIAMethodDataSet": {"shortDescription": [{"value": "Globales Erwärmungspotenzial luluc (GWP-luluc)", "lang": "de"}, {"value": "Global Warming Potential luluc (GWP-luluc)", "lang": "en"}], "type": "LCIA method data set", "refObjectId": "4331bbdb-978a-490d-8707-eeb047f01a55", "uri": "../lciamethods/4331bbdb-978a-490d-8707-eeb047f01a55.xml"}, "other": {"anies": [{"name": "referenceToUnitGroupDataSet", "value": {"shortDescription": [{"value": "kg CO_(2)-Äq.", "lang": "de"}], "type": "unit group data set", "refObjectId": "1ebf3012-d0db-4de2-aefd-ef30cedb0be1", "uri": "../unitgroups/1ebf3012-d0db-4de2-aefd-ef30cedb0be1.xml"}}, {"value": "0.297237042923028", "module": "A1-A3"}, {"value": "0", "module": "C1"}, {"value": "0.00956409139724473", "module": "C2"}, {"value": "0.000737626603965425", "module": "C3"}, {"value": "0", "module": "C4"}, {"value": "-0.0490120307029419", "module": "D"}]}}, {"referenceToLCIAMethodDataSet": {"shortDescription": [{"value": "Abbau Potential der stratosphärischen Ozonschicht (ODP)", "lang": "de"}, {"value": "Depletion potential of the stratospheric ozone layer (ODP)", "lang": "en"}], "type": "LCIA method data set", "refObjectId": "b5c629d6-def3-11e6-bf01-fe55135034f3", "uri": "../lciamethods/b5c629d6-def3-11e6-bf01-fe55135034f3.xml"}, "other": {"anies": [{"name": "referenceToUnitGroupDataSet", "value": {"shortDescription": [{"value": "kg CFC11-Äq.", "lang": "de"}], "type": "unit group data set", "refObjectId": "d9e957c9-7309-4474-bf3a-7777df6c4e5b", "uri": "../unitgroups/d9e957c9-7309-4474-bf3a-7777df6c4e5b.xml"}}, {"value": "8.42434034455497E-10", "module": "A1-A3"}, {"value": "0", "module": "C1"}, {"value": "1.39377260156506E-13", "module": "C2"}, {"value": "5.10536870260145E-11", "module": "C3"}, {"value": "0", "module": "C4"}, {"value": "-3.18276372315642E-09", "module": "D"}]}}, {"referenceToLCIAMethodDataSet": {"shortDescription": [{"value": "Versauerungspotenzial von Boden und Wasser (AP)", "lang": "de"}, {"value": "Acidification potential of land and water (AP)", "lang": "en"}], "type": "LCIA method data set", "refObjectId": "b5c611c6-def3-11e6-bf01-fe55135034f3", "uri": "../lciamethods/b5c611c6-def3-11e6-bf01-fe55135034f3.xml"}, "other": {"anies": [{"name": "referenceToUnitGroupDataSet", "value": {"shortDescription": [{"value": "mol H^(+)-Äq.", "lang": "de"}], "type": "unit group data set", "refObjectId": "42e089ac-92bf-4bf2-8ca1-5fc40d18f2ed", "uri": "../unitgroups/42e089ac-92bf-4bf2-8ca1-5fc40d18f2ed.xml"}}, {"value": "0.674248462856133", "module": "A1-A3"}, {"value": "0", "module": "C1"}, {"value": "0.00474314221098993", "module": "C2"}, {"value": "0.0076583517850452", "module": "C3"}, {"value": "0", "module": "C4"}, {"value": "0.357774641471348", "module": "D"}]}}, {"referenceToLCIAMethodDataSet": {"shortDescription": [{"value": "Eutrophierungspotenzial Süßwasser (EP-freshwater)", "lang": "de"}, {"value": "Eutrophication potential aquatic freshwater (EP-freshwater)", "lang": "en"}], "type": "LCIA method data set", "refObjectId": "b53ec18f-7377-4ad3-86eb-cc3f4f276b2b", "uri": "../lciamethods/b53ec18f-7377-4ad3-86eb-cc3f4f276b2b.xml"}, "other": {"anies": [{"name": "referenceToUnitGroupDataSet", "value": {"shortDescription": [{"value": "kg P-Äq.", "lang": "de"}], "type": "unit group data set", "refObjectId": "0429039d-a61d-4590-ba67-aa4a20a810a1", "uri": "../unitgroups/0429039d-a61d-4590-ba67-aa4a20a810a1.xml"}}, {"value": "0.0022406968623684", "module": "A1-A3"}, {"value": "0", "module": "C1"}, {"value": "5.07017796948572E-06", "module": "C2"}, {"value": "1.01777553760833E-05", "module": "C3"}, {"value": "0", "module": "C4"}, {"value": "-0.000640315294303602", "module": "D"}]}}, {"referenceToLCIAMethodDataSet": {"shortDescription": [{"value": "Eutrophierungspotenzial Salzwasser (EP-marine)", "lang": "de"}, {"value": "Eutrophication potential aquatic marine (EP-marine)", "lang": "en"}], "type": "LCIA method data set", "refObjectId": "b5c619fa-def3-11e6-bf01-fe55135034f3", "uri": "../lciamethods/b5c619fa-def3-11e6-bf01-fe55135034f3.xml"}, "other": {"anies": [{"name": "referenceToUnitGroupDataSet", "value": {"shortDescription": [{"value": "kg N-Äq.", "lang": "de"}], "type": "unit group data set", "refObjectId": "d05bb823-ecdf-4686-8c40-bf1d9257859f", "uri": "../unitgroups/d05bb823-ecdf-4686-8c40-bf1d9257859f.xml"}}, {"value": "0.317409613778038", "module": "A1-A3"}, {"value": "0", "module": "C1"}, {"value": "0.00216878767285638", "module": "C2"}, {"value": "0.00171824713711127", "module": "C3"}, {"value": "0", "module": "C4"}, {"value": "0.0844838694523156", "module": "D"}]}}, {"referenceToLCIAMethodDataSet": {"shortDescription": [{"value": "Eutrophierungspotenzial Land (EP-terrestrial)", "lang": "de"}, {"value": "Eutrophication potential terrestrial (EP-terrestrial)", "lang": "en"}], "type": "LCIA method data set", "refObjectId": "b5c614d2-def3-11e6-bf01-fe55135034f3", "uri": "../lciamethods/b5c614d2-def3-11e6-bf01-fe55135034f3.xml"}, "other": {"anies": [{"name": "referenceToUnitGroupDataSet", "value": {"shortDescription": [{"value": "mol N-Äq.", "lang": "de"}], "type": "unit group data set", "refObjectId": "71b4d617-0ec9-4d3f-b65e-e438940c2401", "uri": "../unitgroups/71b4d617-0ec9-4d3f-b65e-e438940c2401.xml"}}, {"value": "2.94559204384737", "module": "A1-A3"}, {"value": "0", "module": "C1"}, {"value": "0.0242901601351895", "module": "C2"}, {"value": "0.018026668408414", "module": "C3"}, {"value": "0", "module": "C4"}, {"value": "0.990591164294606", "module": "D"}]}}, {"referenceToLCIAMethodDataSet": {"shortDescription": [{"value": "Bildungspotential für troposphärisches Ozon (POCP)", "lang": "de"}, {"value": "Formation potential of tropospheric ozone photochemical oxidants (POCP)", "lang": "en"}], "type": "LCIA method data set", "refObjectId": "b5c610fe-def3-11e6-bf01-fe55135034f3", "uri": "../lciamethods/b5c610fe-def3-11e6-bf01-fe55135034f3.xml"}, "other": {"anies": [{"name": "referenceToUnitGroupDataSet", "value": {"shortDescription": [{"value": "kg NMVOC-Äq.", "lang": "de"}], "type": "unit group data set", "refObjectId": "d27c25f8-fbc1-44c6-b47b-4adbae4199c6", "uri": "../unitgroups/d27c25f8-fbc1-44c6-b47b-4adbae4199c6.xml"}}, {"value": "1.05011570558757", "module": "A1-A3"}, {"value": "0", "module": "C1"}, {"value": "0.00425753547350918", "module": "C2"}, {"value": "0.00464552457008474", "module": "C3"}, {"value": "0", "module": "C4"}, {"value": "0.350725594258857", "module": "D"}]}}, {"referenceToLCIAMethodDataSet": {"shortDescription": [{"value": "Potenzial für den abiotischen Abbau nicht fossiler Ressourcen (ADPE)", "lang": "de"}, {"value": "Abiotic depletion potential for non fossil resources (ADPE)", "lang": "en"}], "type": "LCIA method data set", "refObjectId": "b2ad6494-c78d-11e6-9d9d-cec0c932ce01", "uri": "../lciamethods/b2ad6494-c78d-11e6-9d9d-cec0c932ce01.xml"}, "other": {"anies": [{"name": "referenceToUnitGroupDataSet", "value": {"shortDescription": [{"value": "kg Sb-Äq.", "lang": "de"}], "type": "unit group data set", "refObjectId": "54ccd2d9-a32a-4fc2-923d-f2c8c93e89d4", "uri": "../unitgroups/54ccd2d9-a32a-4fc2-923d-f2c8c93e89d4.xml"}}, {"value": "4.62822797447707E-05", "module": "A1-A3"}, {"value": "0", "module": "C1"}, {"value": "1.4305300289471E-07", "module": "C2"}, {"value": "9.50447878389973E-07", "module": "C3"}, {"value": "0", "module": "C4"}, {"value": "-6.77355076861052E-05", "module": "D"}]}}, {"referenceToLCIAMethodDataSet": {"shortDescription": [{"value": "Potenzial für den abiotischen Abbau fossiler Brennstoffe (ADPF)", "lang": "de"}, {"value": "Abiotic depletion potential for fossil resources (ADPF)", "lang": "en"}], "type": "LCIA method data set", "refObjectId": "b2ad6110-c78d-11e6-9d9d-cec0c932ce01", "uri": "../lciamethods/b2ad6110-c78d-11e6-9d9d-cec0c932ce01.xml"}, "other": {"anies": [{"name": "referenceToUnitGroupDataSet", "value": {"shortDescription": [{"value": "MJ", "lang": "de"}], "type": "unit group data set", "refObjectId": "93a60a57-a3c8-11da-a746-0800200c9a66", "uri": "../unitgroups/93a60a57-a3c8-11da-a746-0800200c9a66.xml"}}, {"value": "1881.15229206553", "module": "A1-A3"}, {"value": "0", "module": "C1"}, {"value": "18.6316096224242", "module": "C2"}, {"value": "63.3231442640325", "module": "C3"}, {"value": "0", "module": "C4"}, {"value": "-6948.55641942906", "module": "D"}]}}, {"referenceToLCIAMethodDataSet": {"shortDescription": [{"value": "Wassernutzung (WDP)", "lang": "de"}, {"value": "Water use (WDP)", "lang": "en"}], "type": "LCIA method data set", "refObjectId": "b2ad66ce-c78d-11e6-9d9d-cec0c932ce01", "uri": "../lciamethods/b2ad66ce-c78d-11e6-9d9d-cec0c932ce01.xml"}, "other": {"anies": [{"name": "referenceToUnitGroupDataSet", "value": {"shortDescription": [{"value": "m^(3) Welt-Äq. entzogen", "lang": "de"}], "type": "unit group data set", "refObjectId": "6ae2df01-888e-46c8-b17d-49fa3869b476", "uri": "../unitgroups/6ae2df01-888e-46c8-b17d-49fa3869b476.xml"}}, {"value": "15.9191344428427", "module": "A1-A3"}, {"value": "0", "module": "C1"}, {"value": "0.0158797032813697", "module": "C2"}, {"value": "0.795445689721902", "module": "C3"}, {"value": "0", "module": "C4"}, {"value": "-22.2378970000827", "module": "D"}]}}, {"referenceToLCIAMethodDataSet": {"shortDescription": [{"value": "Auftreten von Krankheiten aufgrund von Feinstaubemissionen (PM)", "lang": "de"}, {"value": "Incidence of disease due to PM emissions (PM)", "lang": "en"}], "type": "LCIA method data set", "refObjectId": "b5c602c6-def3-11e6-bf01-fe55135034f3", "uri": "../lciamethods/b5c602c6-def3-11e6-bf01-fe55135034f3.xml"}, "other": {"anies": [{"name": "referenceToUnitGroupDataSet", "value": {"shortDescription": [{"value": "Krankheitsfälle", "lang": "de"}], "type": "unit group data set", "refObjectId": "3883559b-648f-4afc-8ba2-0bd24f3affa3", "uri": "../unitgroups/3883559b-648f-4afc-8ba2-0bd24f3affa3.xml"}}, {"module": "A1-A3"}, {"module": "C1"}, {"module": "C2"}, {"module": "C3"}, {"module": "C4"}, {"module": "D"}]}}, {"referenceToLCIAMethodDataSet": {"shortDescription": [{"value": "Wirkung durch Exposition des Menschen mit U235 (IR)", "lang": "de"}, {"value": "Human exposure efficiency relative to U235 (IR)", "lang": "en"}], "type": "LCIA method data set", "refObjectId": "b5c632be-def3-11e6-bf01-fe55135034f3", "uri": "../lciamethods/b5c632be-def3-11e6-bf01-fe55135034f3.xml"}, "other": {"anies": [{"name": "referenceToUnitGroupDataSet", "value": {"shortDescription": [{"value": "kBq U235-Äq.", "lang": "de"}], "type": "unit group data set", "refObjectId": "456b05bf-1415-44a9-9993-02452f554c09", "uri": "../unitgroups/456b05bf-1415-44a9-9993-02452f554c09.xml"}}, {"module": "A1-A3"}, {"module": "C1"}, {"module": "C2"}, {"module": "C3"}, {"module": "C4"}, {"module": "D"}]}}, {"referenceToLCIAMethodDataSet": {"shortDescription": [{"value": "Toxizitätsvergleichseinheit für Ökosysteme (ETP-fw)", "lang": "de"}, {"value": "Comparative toxic unit for ecosystems (ETP-fw)", "lang": "en"}], "type": "LCIA method data set", "refObjectId": "ee1082d1-b0f7-43ca-a1f0-21e2a4a74511", "uri": "../lciamethods/ee1082d1-b0f7-43ca-a1f0-21e2a4a74511.xml"}, "other": {"anies": [{"name": "referenceToUnitGroupDataSet", "value": {"shortDescription": [{"value": "CTUe", "lang": "de"}], "type": "unit group data set", "refObjectId": "aa959ded-f1eb-4efb-9c5c-2d60be36b3e6", "uri": "../unitgroups/aa959ded-f1eb-4efb-9c5c-2d60be36b3e6.xml"}}, {"module": "A1-A3"}, {"module": "C1"}, {"module": "C2"}, {"module": "C3"}, {"module": "C4"}, {"module": "D"}]}}, {"referenceToLCIAMethodDataSet": {"shortDescription": [{"value": "Toxizitätsvergleichseinheit für Menschen (krebserregend) (HTP-c)", "lang": "de"}, {"value": "Comparative toxic unit for humans (carcinogenic) (HTP-c)", "lang": "en"}], "type": "LCIA method data set", "refObjectId": "2299222a-bbd8-474f-9d4f-4dd1f18aea7c", "uri": "../lciamethods/2299222a-bbd8-474f-9d4f-4dd1f18aea7c.xml"}, "other": {"anies": [{"name": "referenceToUnitGroupDataSet", "value": {"shortDescription": [{"value": "CTUh", "lang": "de"}], "type": "unit group data set", "refObjectId": "d4c9523e-2d7e-49fd-8469-998f547d3a70", "uri": "../unitgroups/d4c9523e-2d7e-49fd-8469-998f547d3a70.xml"}}, {"module": "A1-A3"}, {"module": "C1"}, {"module": "C2"}, {"module": "C3"}, {"module": "C4"}, {"module": "D"}]}}, {"referenceToLCIAMethodDataSet": {"shortDescription": [{"value": "Toxizitätsvergleichseinheit für Menschen (nicht krebserregend) (HTP-nc)", "lang": "de"}, {"value": "Comparative toxic unit for humans (noncarcinogenic) (HTP-nc)", "lang": "en"}], "type": "LCIA method data set", "refObjectId": "3af763a5-b7a1-48c9-9cee-1f223481fcef", "uri": "../lciamethods/3af763a5-b7a1-48c9-9cee-1f223481fcef.xml"}, "other": {"anies": [{"name": "referenceToUnitGroupDataSet", "value": {"shortDescription": [{"value": "CTUh", "lang": "de"}], "type": "unit group data set", "refObjectId": "d4c9523e-2d7e-49fd-8469-998f547d3a70", "uri": "../unitgroups/d4c9523e-2d7e-49fd-8469-998f547d3a70.xml"}}, {"module": "A1-A3"}, {"module": "C1"}, {"module": "C2"}, {"module": "C3"}, {"module": "C4"}, {"module": "D"}]}}, {"referenceToLCIAMethodDataSet": {"shortDescription": [{"value": "Bodenqualitätsindex (SQP)", "lang": "de"}, {"value": "Soil quality index (SQP)", "lang": "en"}], "type": "LCIA method data set", "refObjectId": "b2ad6890-c78d-11e6-9d9d-cec0c932ce01", "uri": "../lciamethods/b2ad6890-c78d-11e6-9d9d-cec0c932ce01.xml"}, "other": {"anies": [{"name": "referenceToUnitGroupDataSet", "value": {"shortDescription": [{"value": "SQP", "lang": "de"}], "type": "unit group data set", "refObjectId": "f130951c-e67f-4f7f-8dd4-665de3974e18", "uri": "../unitgroups/f130951c-e67f-4f7f-8dd4-665de3974e18.xml"}}, {"module": "A1-A3"}, {"module": "C1"}, {"module": "C2"}, {"module": "C3"}, {"module": "C4"}, {"module": "D"}]}}]}, "otherAttributes": {"{http://www.indata.network/EPD/2019}epd-version": "1.2"}, "version": "1.1", "locations": "../ILCDLocations.xml"}