{"processInformation": {"dataSetInformation": {"UUID": "5f025d1f-cf04-4ccb-8495-6a2c58647b96", "name": {"baseName": [{"value": "ES PROLINE", "lang": "en"}, {"value": "ES PROLINE", "lang": "de"}], "functionalUnitFlowProperties": [{"lang": "en"}]}, "classificationInformation": {"classification": [{"class": [{"value": "Komponenten von Fenstern und Vorhangfassaden", "level": 0, "classId": "7"}, {"value": "Antriebssysteme", "level": 1, "classId": "7.7"}, {"value": "elektrisch", "level": 2, "classId": "7.7.02"}], "name": "OEKOBAU.DAT"}, {"class": [{"value": "02 Building products", "level": 0}, {"value": "Doors, windows, shutters, and related products", "level": 1}, {"value": "Drive systems for automatic doors and gates", "level": 2}], "name": "IBUCategories"}]}, "generalComment": [{"value": "With ES PROLINE, a drive system has been developed that offers the latest dormakaba technology.\nAt the same time, the drive meets high design and functional requirements of modern buildings.\nThe ES PROLINE drive system offers versatile application possibilities. It does not matter whether it is a standard door, a door in escape and rescue routes or a telescopic sliding door.\nEven particularly heavy door leaves are no problem for the drive. Up to 400 kg can be moved with the new system.\nWith the following ES PROLINE drive system variants you can meet almost all requirements:\n\nES 250: Standard doors \nES 250 PRO FST: Escape and rescue routes \nES 250 PRO EASY: Standard doors, less features\nES 400 PRO / ES 400 PRO FST: For heavy standard doors and escape and rescue routes optional with Resistance Class (RC) The product family of the modular automatic ES PROLINE drive system covers all above mentioned drive systems. The configuration of the drive is modular. Additional modules can be added like battery packs and interlocks. Values (material and energy flows) for a representative product are based on the volumes of ES PROLINE variants sold during the reference period.\nFor the placing on the market in the European Union/European Free Trade Associaton (EU/EFTA) (with the exception of Switzerland) the following legal provisions apply:\n\nMachinery Directive 2006/42/EC\n2014/30/EU Electromagnetic Compatibility Directive\n2011/65/EU ROHS3 Directive\nDIN EN ISO 12100:2011-03 Safety of machinery\nDIN EN 16005: 2013-01 and Amendment 2015-10 Power operated pedestrian doorsets\nDIN EN ISO 13849- 1:2016-06 Safety of machinery\nDIN EN 60335-2-103: 2016-05 Household and similar electrical appliances\nDIN EN 61000-3-2:2015-03 Electromagnetic compatibility (EMC)\nDIN EN 61000-3-3: 2014-03 Electromagnetic compatibility (EMC)\nDIN EN 61000-6-2: 2005 and Amendment:2011 Electromagnetic Compatibility (EMC)\nDIN EN 61000-6-3:2007 and A1:2011 Electromagnetic Compatibility (EMC)\nDIN EN IEC 63000: 2019-05The CE-marking takes into account the proof of conformity with the respective harmonized standards based on the legal provisions above.", "lang": "en"}, {"value": "Mit ES PROLINE wurde ein Antriebssystem entwickelt, das die neueste dormakaba Technologie bietet. Gleichzeitig erfüllt der Antrieb hohe Design- und Funktionsanforderungen moderner Gebäude. Das ES PROLINE Antriebssystem bietet vielseitige Einsatzmöglichkeiten. Ganz gleich, ob es sich um eine Standardtür, eine Tür in Flucht- und Rettungswegen oder eine Teleskopschiebetür handelt. Auch besonders schwere Türflügel sind für den Antrieb kein Problem. Bis zu 400 kg können mit dem neuen System bewegt werden. Mit den folgenden Varianten des ES PROLINE Antriebssystems können Sie fast alle Anforderungen erfüllen: ES 250: Standardtüren ES 250 PRO FST: Flucht- und Rettungswege ES 250 PRO EASY: Standardtüren, weniger Ausstattung ES 400 PRO / ES 400 PRO FST: Für schwere Standardtüren und Flucht- und Rettungswege optional mit Resistance Class (RC) Die Produktfamilie des modularen automatischen ES PROLINE Antriebssystems umfasst alle oben genannten Antriebssysteme. Die Konfiguration des Antriebs ist modular. Es können zusätzliche Module wie Akkupacks und Verriegelungen hinzugefügt werden. Die Werte (Material- und Energieströme) für ein repräsentatives Produkt basieren auf dem Volumen der im Bezugszeitraum verkauften ES PROLINE Varianten.\nFür das Inverkehrbringen in der Europäischen Union/Europäischen Freihandelsassoziation (EU/EFTA) (mit Ausnahme der Schweiz) gelten folgende gesetzliche Bestimmungen: Maschinenrichtlinie 2006/42/EG 2014/30/EU Richtlinie über elektromagnetische Verträglichkeit 2011/65/EU ROHS3-Richtlinie DIN EN ISO 12100:2011-03 Sicherheit von Maschinen DIN EN 16005: 2013-01 und Änderung 2015-10 Kraftbetätigte Fußgängertüren DIN EN ISO 13849- 1:2016-06 Sicherheit von Maschinen DIN EN 60335-2-103: 2016-05 Elektrische Geräte für den Hausgebrauch und ähnliche Zwecke DIN EN 61000-3-2:2015-03 Elektromagnetische Verträglichkeit (EMV) DIN EN 61000-3-3: 2014-03 Elektromagnetische Verträglichkeit (EMV) DIN EN 61000-6-2: 2005 und Änderung:2011 Elektromagnetische Verträglichkeit (EMV) DIN EN 61000-6-3:2007 und A1:2011 Elektromagnetische Verträglichkeit (EMV) DIN EN IEC 63000: 2019-05Die CE-Kennzeichnung berücksichtigt den Nachweis der Konformität mit den jeweiligen harmonisierten Normen auf der Grundlage der oben genannten gesetzlichen Bestimmungen.", "lang": "de"}]}, "quantitativeReference": {"referenceToReferenceFlow": [0]}, "time": {"referenceYear": 2021, "dataSetValidUntil": 2026, "other": {"anies": [{"name": "publicationDateOfEPD", "value": 1624838400000}]}}, "geography": {"locationOfOperationSupplyOrProduction": {"location": "DE"}}, "technology": {"technologyDescriptionAndIncludedProcesses": [{"value": "The drive units and requisite circuit boards of ES PROLINE product family are manufactured at dormakaba. The certified Quality Management system in accordance with ISO 9001 safeguards the high-quality standard of dormakaba products. It guarantees continuous improvement of the overall processes and product quality at the dormakaba locations. \nTechnical data: \nThe following technical data is of relevance for the LCA: \nDeclared unit: \nThe declaration represents one (1) ES PROLINE.", "lang": "en"}, {"value": "Die Antriebseinheiten und die dazugehörigen Leiterplatten der ES PROLINE Produktfamilie werden bei dormakaba gefertigt. Das zertifizierte Qualitätsmanagementsystem nach ISO 9001 sichert den hohen Qualitätsstandard der dormakaba Produkte. Es garantiert eine kontinuierliche Verbesserung der Gesamtprozesse und der Produktqualität an den dormakaba Standorten. \nTechnische Daten: \nDie folgenden technischen Daten sind für die LCA von Bedeutung: \nDeklarierte Einheit: \nDie Erklärung steht für eine (1) ES PROLINE.", "lang": "de"}], "technologicalApplicability": [{"value": "The automatic ES PROLINE drive system is used as a drive for automating sliding door systems as well as escape and rescue routes:", "lang": "en"}, {"value": "Das automatische Antriebssystem ES PROLINE wird als Antrieb für die Automatisierung von Schiebetürsystemen sowie Flucht- und Rettungswegen eingesetzt:", "lang": "de"}]}}, "modellingAndValidation": {"LCIMethodAndAllocation": {"typeOfDataSet": "EPD", "referenceToLCAMethodDetails": [{"shortDescription": [{"value": "Drive systems for automatic doors and gates.pdf", "lang": "en"}], "type": "source data set", "refObjectId": "fa2fd5d8-91c3-48c8-b733-44afd294b93c"}], "other": {"anies": [{"name": "subType", "value": "specific dataset"}]}}, "dataSourcesTreatmentAndRepresentativeness": {"referenceToDataSource": [{"shortDescription": [{"value": "GaBi Database (all versions)", "lang": "en"}], "type": "source data set", "refObjectId": "28d74cc0-db8b-4d7e-bc44-5f6d56ce0c4a"}, {"shortDescription": [{"value": "GaBi database SP40 2020", "lang": "en"}], "type": "source data set", "refObjectId": "0115289e-52f0-4920-bc7e-57b1c96aec8d"}], "useAdviceForDataSet": [{"value": "Scope: \nThis EPD refers to the entire life cycle of a representative ES PROLINE drive system.\nThe various technical characteristics are depicted in section 2.3.\nThe production location is the DORMA production site in Ennepetal, Germany.\nThe material and energy flows were taken into consideration accordingly. \nSystem boundary: \nType of the EPD: cradle to gate - with options Modules A1-A3, A4, and A5\nThe product stage (A1-A3) begins with considering the production of the necessary raw materials and energies, including all corresponding upstream chains and the actual procurement transports. Furthermore, the entire manufacturing phase was mapped, including the treatment of production waste until the end-of-waste status (EoW) was reached. In addition, both the distribution transports (A4) and the installation including power-consuming tools, installation materials and the packaging waste generated during installation (A5) were taken into account. \n\nModule B6\nModule B6 includes the operational energy use over the service life of 15 years.\n\nModules C1-C4\nThe modules include the environmental impacts for dismantling of the ES PROLINE and the treatment of the waste categories until end-of-waste status (EoW) is reached, including the associated transports at the end of the product life cycle.\n\nModule D\nIdentification of the benefits and costs of the product outside the system boundary. For plastics, these consist of energy credits from thermal utilization (C3) in the form of the average European electricity mix or thermal energy from natural gas. Recycling of metal scrap results in credits of the respective raw materials.", "lang": "en"}, {"value": "Gültigkeitsbereich: \nDiese EPD bezieht sich auf den gesamten Lebenszyklus eines repräsentativen ES PROLINE Antriebssystems. Die verschiedenen technischen Merkmale sind in Abschnitt 2.3 dargestellt. Der Produktionsstandort ist die DORMA Produktionsstätte in Ennepetal, Deutschland. Die Stoff- und Energieströme wurden entsprechend berücksichtigt. \nSystemgrenze: \nArt der EPD: cradle to gate - mit Optionen Module A1-A3, A4 und A5 Die Produktphase (A1-A3) beginnt mit der Betrachtung der Herstellung der benötigten Rohstoffe und Energien, einschließlich aller entsprechenden Vorketten und der eigentlichen Beschaffungstransporte. Außerdem wurde die gesamte Herstellungsphase abgebildet, einschließlich der Behandlung von Produktionsabfällen bis zum Erreichen des End-of-Waste-Status (EoW). Darüber hinaus wurden sowohl die Verteilungstransporte (A4) als auch die Installation einschließlich der stromverbrauchenden Werkzeuge, der Installationsmaterialien und der bei der Installation anfallenden Verpackungsabfälle (A5) berücksichtigt. \n\nModul B6 Modul B6 umfasst den betrieblichen Energieverbrauch über die Nutzungsdauer von 15 Jahren. Module C1-C4 Die Module umfassen die Umweltauswirkungen für die Demontage der ES PROLINE und die Behandlung der Abfallkategorien bis zum Erreichen des End-of-Waste-Status (EoW), einschließlich der damit verbundenen Transporte am Ende des Produktlebenszyklus. Modul D Identifizierung der Vorteile und Kosten des Produkts außerhalb der Systemgrenze. Bei Kunststoffen bestehen diese aus Energiegutschriften aus der thermischen Verwertung (C3) in Form des durchschnittlichen europäischen Strommixes oder thermischer Energie aus Erdgas. Das Recycling von Metallschrott führt zu Gutschriften für die entsprechenden Rohstoffe.", "lang": "de"}], "other": {"anies": [{"name": "referenceToOriginalEPD", "value": {"shortDescription": {"value": "ES PROLINE.pdf", "defaultValue": "ES PROLINE.pdf", "lstrings": [{"lang": "en", "value": "ES PROLINE.pdf"}]}, "type": "source data set", "uuid": {"uuid": "5cdcce20-2866-485c-8e83-38386410e097"}, "refObjectId": "5cdcce20-2866-485c-8e83-38386410e097", "resourceURLs": ["https://oekobaudat.de/OEKOBAU.DAT/resource/sources/5cdcce20-2866-485c-8e83-38386410e097/ES_PROLINE_23929.pdf?version=00.03.000"]}}]}}, "validation": {"review": [{"referenceToNameOfReviewerAndInstitution": [{"shortDescription": [{"value": "Institut Bauen und Umwelt e. V.", "lang": "en"}], "type": "contact data set", "refObjectId": "d111dbec-b024-4be5-86c5-752d6eb2cf95", "uri": "../contacts/d111dbec-b024-4be5-86c5-752d6eb2cf95.xml"}], "type": "Accredited third party review"}]}, "complianceDeclarations": {"compliance": [{"referenceToComplianceSystem": {"shortDescription": [{"value": "DIN EN 15804", "lang": "en"}], "type": "source data set", "refObjectId": "b00f9ec0-7874-11e3-981f-0800200c9a66", "uri": "../sources/b00f9ec0-7874-11e3-981f-0800200c9a66.xml"}}, {"referenceToComplianceSystem": {"shortDescription": [{"value": "ISO 14025", "lang": "en"}], "type": "source data set", "refObjectId": "4f2eb655-6e44-4874-a95a-e28f5442cd4d", "uri": "../sources/4f2eb655-6e44-4874-a95a-e28f5442cd4d.xml"}}]}}, "administrativeInformation": {"commissionerAndGoal": {"referenceToCommissioner": [{"shortDescription": [{"value": "dormakaba International Holding GmbH", "lang": "en"}], "type": "contact data set", "refObjectId": "33313944-7b37-498a-b458-25a295c1017d", "uri": "../contacts/33313944-7b37-498a-b458-25a295c1017d.xml"}]}, "dataGenerator": {"referenceToPersonOrEntityGeneratingTheDataSet": [{"shortDescription": [{"value": "brands and values GmbH", "lang": "en"}], "type": "contact data set", "refObjectId": "6b539b8a-10e3-4004-8ccc-a79f169aa339", "uri": "../contacts/6b539b8a-10e3-4004-8ccc-a79f169aa339.xml"}]}, "dataEntryBy": {"timeStamp": 1624838400000, "referenceToDataSetFormat": [{"shortDescription": [{"value": "ILCD Format", "lang": "en"}], "type": "source data set", "refObjectId": "a97a0155-0234-4b87-b4ce-a45da52f2a40", "uri": "../sources/a97a0155-0234-4b87-b4ce-a45da52f2a40.xml"}, {"shortDescription": [{"value": "EPD-Datenformaterweiterungen v1.2", "lang": "de"}, {"value": "EPD Data Format Extensions v1.2", "lang": "en"}], "type": "source data set", "refObjectId": "a29449fd-aa2f-4de8-b5d7-4b06b43c6fde", "uri": "../sources/a29449fd-aa2f-4de8-b5d7-4b06b43c6fde.xml"}]}, "publicationAndOwnership": {"dataSetVersion": "00.01.000", "referenceToRegistrationAuthority": {"shortDescription": [{"value": "Institut Bauen und Umwelt e. V.", "lang": "en"}], "type": "contact data set", "refObjectId": "d111dbec-b024-4be5-86c5-752d6eb2cf95", "uri": "../contacts/d111dbec-b024-4be5-86c5-752d6eb2cf95.xml"}, "registrationNumber": "EPD-DOR-20200269-IBA1-EN", "referenceToOwnershipOfDataSet": {"shortDescription": [{"value": "dormakaba International Holding GmbH", "lang": "en"}], "type": "contact data set", "refObjectId": "33313944-7b37-498a-b458-25a295c1017d", "uri": "../contacts/33313944-7b37-498a-b458-25a295c1017d.xml"}, "copyright": true, "licenseType": "Free of charge for all users and uses", "accessRestrictions": [{"value": "None", "lang": "en"}], "other": {"anies": [{"name": "referenceToPublisher", "value": {"shortDescription": [{"value": "Institut Bauen und Umwelt e. V.", "lang": "en"}], "type": "contact data set", "refObjectId": "d111dbec-b024-4be5-86c5-752d6eb2cf95", "uri": "../contacts/d111dbec-b024-4be5-86c5-752d6eb2cf95.xml"}}]}}}, "exchanges": {"exchange": [{"dataSetInternalID": 0, "referenceToFlowDataSet": {"shortDescription": [{"value": "ES PROLINE (ES PROLINE)", "lang": "en"}], "type": "flow data set", "refObjectId": "707c63fe-e172-b5e5-c9f1-762502f1dad1", "uri": "../flows/707c63fe-e172-b5e5-c9f1-762502f1dad1.xml"}, "meanAmount": 1.0, "referencesToDataSource": {}, "referenceFlow": true, "resolvedFlowVersion": "00.01.000", "resultingflowAmount": 1.0, "flowProperties": [{"name": [{"lang": "de", "value": "Anzahl"}, {"lang": "en", "value": "Number of pieces"}], "uuid": "01846770-4cfe-4a25-8ad9-919d8d378345", "referenceFlowProperty": true, "meanValue": 1.0, "referenceUnit": "pcs.", "unitGroupUUID": "934110e3-baf4-49e9-992c-3d8109a6aafb"}], "materialProperties": [{"name": "weight per piece", "value": "27.47", "unit": "kg"}], "typeOfFlow": "Product flow", "classification": {"classHierarchy": "Komponenten von Fenstern und Vorhangfassaden / Antriebssysteme / elektrisch", "name": "OEKOBAU.DAT"}}, {"dataSetInternalID": 1, "referenceToFlowDataSet": {"shortDescription": [{"value": "Renewable primary energy as energy carrier (PERE)", "lang": "en"}, {"value": "Erneuerbare Primärenergie als Energieträger (PERE)", "lang": "de"}], "type": "flow data set", "refObjectId": "20f32be5-0398-4288-9b6d-accddd195317", "uri": "../flows/20f32be5-0398-4288-9b6d-accddd195317.xml"}, "exchange direction": "INPUT", "other": {"anies": [{"name": "referenceToUnitGroupDataSet", "value": {"shortDescription": [{"value": "MJ", "lang": "en"}], "type": "unit group data set", "refObjectId": "93a60a57-a3c8-11da-a746-0800200c9a66", "uri": "../unitgroups/93a60a57-a3c8-11da-a746-0800200c9a66.xml"}}, {"value": "380.2976", "module": "A1-A3"}, {"value": "1.23", "module": "A4"}, {"value": "38.7224", "module": "A5"}, {"value": "3100", "module": "B6"}, {"value": "0.0327", "module": "C1"}, {"value": "0.171", "module": "C2"}, {"value": "0.878", "module": "C3"}, {"value": "0", "module": "C4"}, {"value": "-132", "module": "D"}]}, "resolvedFlowVersion": "38.00.000", "flowProperties": [], "typeOfFlow": "Other flow", "classification": {"classHierarchy": "Quantities", "name": "GaBiCategories"}}, {"dataSetInternalID": 2, "referenceToFlowDataSet": {"shortDescription": [{"value": "Renewable primary energy resources as material utilization (PERM)", "lang": "en"}, {"value": "Erneuerbare Primärenergie zur stofflichen Nutzung (PERM)", "lang": "de"}], "type": "flow data set", "refObjectId": "fb3ec0de-548d-4508-aea5-00b73bf6f702", "uri": "../flows/fb3ec0de-548d-4508-aea5-00b73bf6f702.xml"}, "exchange direction": "INPUT", "other": {"anies": [{"name": "referenceToUnitGroupDataSet", "value": {"shortDescription": [{"value": "MJ", "lang": "en"}], "type": "unit group data set", "refObjectId": "93a60a57-a3c8-11da-a746-0800200c9a66", "uri": "../unitgroups/93a60a57-a3c8-11da-a746-0800200c9a66.xml"}}, {"value": "37.7024", "module": "A1-A3"}, {"value": "0", "module": "A4"}, {"value": "-37.7024", "module": "A5"}, {"value": "0", "module": "B6"}, {"value": "0", "module": "C1"}, {"value": "0", "module": "C2"}, {"value": "0", "module": "C3"}, {"value": "0", "module": "C4"}, {"value": "0", "module": "D"}]}, "resolvedFlowVersion": "38.00.000", "flowProperties": [], "typeOfFlow": "Other flow", "classification": {"classHierarchy": "Quantities", "name": "GaBiCategories"}}, {"dataSetInternalID": 3, "referenceToFlowDataSet": {"shortDescription": [{"value": "Total use of renewable primary energy resources (PERT)", "lang": "en"}, {"value": "Total erneuerbare Primärenergie (PERT)", "lang": "de"}], "type": "flow data set", "refObjectId": "53f97275-fa8a-4cdd-9024-65936002acd0", "uri": "../flows/53f97275-fa8a-4cdd-9024-65936002acd0.xml"}, "exchange direction": "INPUT", "other": {"anies": [{"name": "referenceToUnitGroupDataSet", "value": {"shortDescription": [{"value": "MJ", "lang": "en"}], "type": "unit group data set", "refObjectId": "93a60a57-a3c8-11da-a746-0800200c9a66", "uri": "../unitgroups/93a60a57-a3c8-11da-a746-0800200c9a66.xml"}}, {"value": "418", "module": "A1-A3"}, {"value": "1.23", "module": "A4"}, {"value": "1.02", "module": "A5"}, {"value": "3100", "module": "B6"}, {"value": "0.0327", "module": "C1"}, {"value": "0.171", "module": "C2"}, {"value": "0.878", "module": "C3"}, {"value": "0", "module": "C4"}, {"value": "-132", "module": "D"}]}, "resolvedFlowVersion": "38.00.000", "flowProperties": [], "typeOfFlow": "Other flow", "classification": {"classHierarchy": "Quantities / Environmental quantities / EPD EN 15804 / LCI indicators", "name": "GaBiCategories"}}, {"dataSetInternalID": 4, "referenceToFlowDataSet": {"shortDescription": [{"value": "Non renewable primary energy as energy carrier (PENRE)", "lang": "en"}, {"value": "Nicht-erneuerbare Primärenergie als Energieträger (PENRE)", "lang": "de"}], "type": "flow data set", "refObjectId": "ac857178-2b45-46ec-892a-a9a4332f0372", "uri": "../flows/ac857178-2b45-46ec-892a-a9a4332f0372.xml"}, "exchange direction": "INPUT", "other": {"anies": [{"name": "referenceToUnitGroupDataSet", "value": {"shortDescription": [{"value": "MJ", "lang": "en"}], "type": "unit group data set", "refObjectId": "93a60a57-a3c8-11da-a746-0800200c9a66", "uri": "../unitgroups/93a60a57-a3c8-11da-a746-0800200c9a66.xml"}}, {"value": "2900.73844", "module": "A1-A3"}, {"value": "36.2", "module": "A4"}, {"value": "8.224", "module": "A5"}, {"value": "7000", "module": "B6"}, {"value": "0.0737", "module": "C1"}, {"value": "2.93", "module": "C2"}, {"value": "93.04713", "module": "C3"}, {"value": "0", "module": "C4"}, {"value": "-397", "module": "D"}]}, "resolvedFlowVersion": "38.00.000", "flowProperties": [], "typeOfFlow": "Other flow", "classification": {"classHierarchy": "Quantities", "name": "GaBiCategories"}}, {"dataSetInternalID": 5, "referenceToFlowDataSet": {"shortDescription": [{"value": "Non renewable primary energy as material utilization (PENRM)", "lang": "en"}, {"value": "Nicht-erneuerbare Primärenergie zur stofflichen Nutzung (PENRM)", "lang": "de"}], "type": "flow data set", "refObjectId": "1421caa0-679d-4bf4-b282-0eb850ccae27", "uri": "../flows/1421caa0-679d-4bf4-b282-0eb850ccae27.xml"}, "exchange direction": "INPUT", "other": {"anies": [{"name": "referenceToUnitGroupDataSet", "value": {"shortDescription": [{"value": "MJ", "lang": "en"}], "type": "unit group data set", "refObjectId": "93a60a57-a3c8-11da-a746-0800200c9a66", "uri": "../unitgroups/93a60a57-a3c8-11da-a746-0800200c9a66.xml"}}, {"value": "89.26156", "module": "A1-A3"}, {"value": "0", "module": "A4"}, {"value": "-0.344", "module": "A5"}, {"value": "0", "module": "B6"}, {"value": "0", "module": "C1"}, {"value": "0", "module": "C2"}, {"value": "-88.91713", "module": "C3"}, {"value": "0", "module": "C4"}, {"value": "0", "module": "D"}]}, "resolvedFlowVersion": "38.00.000", "flowProperties": [], "typeOfFlow": "Other flow", "classification": {"classHierarchy": "Quantities", "name": "GaBiCategories"}}, {"dataSetInternalID": 6, "referenceToFlowDataSet": {"shortDescription": [{"value": "Total use of non renewable primary energy resources (PENRT)", "lang": "en"}, {"value": "Total nicht erneuerbare Primärenergie (PENRT)", "lang": "de"}], "type": "flow data set", "refObjectId": "06159210-646b-4c8d-8583-da9b3b95a6c1", "uri": "../flows/06159210-646b-4c8d-8583-da9b3b95a6c1.xml"}, "exchange direction": "INPUT", "other": {"anies": [{"name": "referenceToUnitGroupDataSet", "value": {"shortDescription": [{"value": "MJ", "lang": "en"}], "type": "unit group data set", "refObjectId": "93a60a57-a3c8-11da-a746-0800200c9a66", "uri": "../unitgroups/93a60a57-a3c8-11da-a746-0800200c9a66.xml"}}, {"value": "2990", "module": "A1-A3"}, {"value": "36.2", "module": "A4"}, {"value": "7.88", "module": "A5"}, {"value": "7000", "module": "B6"}, {"value": "0.0737", "module": "C1"}, {"value": "2.93", "module": "C2"}, {"value": "4.13", "module": "C3"}, {"value": "0", "module": "C4"}, {"value": "-397", "module": "D"}]}, "resolvedFlowVersion": "38.00.000", "flowProperties": [], "typeOfFlow": "Other flow", "classification": {"classHierarchy": "Quantities / Environmental quantities / EPD EN 15804 / LCI indicators", "name": "GaBiCategories"}}, {"dataSetInternalID": 7, "referenceToFlowDataSet": {"shortDescription": [{"value": "Use of secondary material (SM)", "lang": "en"}, {"value": "Einsatz von Sekundärstoffen (SM)", "lang": "de"}], "type": "flow data set", "refObjectId": "c6a1f35f-2d09-4f54-8dfb-97e502e1ce92", "uri": "../flows/c6a1f35f-2d09-4f54-8dfb-97e502e1ce92.xml"}, "exchange direction": "INPUT", "other": {"anies": [{"name": "referenceToUnitGroupDataSet", "value": {"shortDescription": [{"value": "kg", "lang": "en"}], "type": "unit group data set", "refObjectId": "ad38d542-3fe9-439d-9b95-2f5f7752acaf", "uri": "../unitgroups/ad38d542-3fe9-439d-9b95-2f5f7752acaf.xml"}}, {"value": "14.3228874208", "module": "A1-A3"}, {"value": "0", "module": "A4"}, {"value": "0", "module": "A5"}, {"value": "0", "module": "B6"}, {"value": "0", "module": "C1"}, {"value": "0", "module": "C2"}, {"value": "0", "module": "C3"}, {"value": "0", "module": "C4"}, {"value": "9.6", "module": "D"}]}, "resolvedFlowVersion": "38.00.000", "flowProperties": [], "typeOfFlow": "Other flow", "classification": {"classHierarchy": "Quantities / Environmental quantities / EPD EN 15804 / LCI indicators", "name": "GaBiCategories"}}, {"dataSetInternalID": 8, "referenceToFlowDataSet": {"shortDescription": [{"value": "Use of renewable secondary fuels (RSF)", "lang": "en"}, {"value": "Erneuerbare Sekundärbrennstoffe (RSF)", "lang": "de"}], "type": "flow data set", "refObjectId": "64333088-a55f-4aa2-9a31-c10b07816787", "uri": "../flows/64333088-a55f-4aa2-9a31-c10b07816787.xml"}, "exchange direction": "INPUT", "other": {"anies": [{"name": "referenceToUnitGroupDataSet", "value": {"shortDescription": [{"value": "MJ", "lang": "en"}], "type": "unit group data set", "refObjectId": "93a60a57-a3c8-11da-a746-0800200c9a66", "uri": "../unitgroups/93a60a57-a3c8-11da-a746-0800200c9a66.xml"}}, {"value": "0", "module": "A1-A3"}, {"value": "0", "module": "A4"}, {"value": "0", "module": "A5"}, {"value": "0", "module": "B6"}, {"value": "0", "module": "C1"}, {"value": "0", "module": "C2"}, {"value": "0", "module": "C3"}, {"value": "0", "module": "C4"}, {"value": "0", "module": "D"}]}, "resolvedFlowVersion": "38.00.000", "flowProperties": [], "typeOfFlow": "Other flow", "classification": {"classHierarchy": "Quantities / Environmental quantities / EPD EN 15804 / LCI indicators", "name": "GaBiCategories"}}, {"dataSetInternalID": 9, "referenceToFlowDataSet": {"shortDescription": [{"value": "Use of non renewable secondary fuels (NRSF)", "lang": "en"}, {"value": "Nicht erneuerbare Sekundärbrennstoffe (NRSF)", "lang": "de"}], "type": "flow data set", "refObjectId": "89def144-d39a-4287-b86f-efde453ddcb2", "uri": "../flows/89def144-d39a-4287-b86f-efde453ddcb2.xml"}, "exchange direction": "INPUT", "other": {"anies": [{"name": "referenceToUnitGroupDataSet", "value": {"shortDescription": [{"value": "MJ", "lang": "en"}], "type": "unit group data set", "refObjectId": "93a60a57-a3c8-11da-a746-0800200c9a66", "uri": "../unitgroups/93a60a57-a3c8-11da-a746-0800200c9a66.xml"}}, {"value": "0", "module": "A1-A3"}, {"value": "0", "module": "A4"}, {"value": "0", "module": "A5"}, {"value": "0", "module": "B6"}, {"value": "0", "module": "C1"}, {"value": "0", "module": "C2"}, {"value": "0", "module": "C3"}, {"value": "0", "module": "C4"}, {"value": "0", "module": "D"}]}, "resolvedFlowVersion": "38.00.000", "flowProperties": [], "typeOfFlow": "Other flow", "classification": {"classHierarchy": "Quantities / Environmental quantities / EPD EN 15804 / LCI indicators", "name": "GaBiCategories"}}, {"dataSetInternalID": 10, "referenceToFlowDataSet": {"shortDescription": [{"value": "Use of net fresh water (FW)", "lang": "en"}, {"value": "Einsatz von Süßwasserressourcen (FW)", "lang": "de"}], "type": "flow data set", "refObjectId": "3cf952c8-f3a4-461d-8c96-96456ca62246", "uri": "../flows/3cf952c8-f3a4-461d-8c96-96456ca62246.xml"}, "exchange direction": "INPUT", "other": {"anies": [{"name": "referenceToUnitGroupDataSet", "value": {"shortDescription": [{"value": "m^3", "lang": "en"}], "type": "unit group data set", "refObjectId": "cd950537-0a98-4044-9ba7-9f9a68d0a504", "uri": "../unitgroups/cd950537-0a98-4044-9ba7-9f9a68d0a504.xml"}}, {"value": "6.508", "module": "A1-A3"}, {"value": "0.00145", "module": "A4"}, {"value": "0.0136", "module": "A5"}, {"value": "3.59", "module": "B6"}, {"value": "3.78E-05", "module": "C1"}, {"value": "0.000184", "module": "C2"}, {"value": "0.0185", "module": "C3"}, {"value": "0", "module": "C4"}, {"value": "-0.361", "module": "D"}]}, "resolvedFlowVersion": "38.00.000", "flowProperties": [], "typeOfFlow": "Other flow", "classification": {"classHierarchy": "Quantities / Environmental quantities / EPD EN 15804 / LCI indicators", "name": "GaBiCategories"}}, {"dataSetInternalID": 11, "referenceToFlowDataSet": {"shortDescription": [{"value": "Hazardous waste disposed (HWD)", "lang": "en"}, {"value": "Gefährlicher Abfall zur Deponie (HWD)", "lang": "de"}], "type": "flow data set", "refObjectId": "430f9e0f-59b2-46a0-8e0d-55e0e84948fc", "uri": "../flows/430f9e0f-59b2-46a0-8e0d-55e0e84948fc.xml"}, "exchange direction": "OUTPUT", "other": {"anies": [{"name": "referenceToUnitGroupDataSet", "value": {"shortDescription": [{"value": "kg", "lang": "en"}], "type": "unit group data set", "refObjectId": "ad38d542-3fe9-439d-9b95-2f5f7752acaf", "uri": "../unitgroups/ad38d542-3fe9-439d-9b95-2f5f7752acaf.xml"}}, {"value": "9.58E-06", "module": "A1-A3"}, {"value": "9.76E-07", "module": "A4"}, {"value": "2.27E-08", "module": "A5"}, {"value": "2.9E-06", "module": "B6"}, {"value": "3.05E-11", "module": "C1"}, {"value": "1.27E-07", "module": "C2"}, {"value": "1.55E-08", "module": "C3"}, {"value": "0", "module": "C4"}, {"value": "-1.17E-07", "module": "D"}]}, "resolvedFlowVersion": "38.00.000", "flowProperties": [], "typeOfFlow": "Other flow", "classification": {"classHierarchy": "Quantities / Environmental quantities / EPD EN 15804 / LCI indicators", "name": "GaBiCategories"}}, {"dataSetInternalID": 12, "referenceToFlowDataSet": {"shortDescription": [{"value": "Non hazardous waste disposed (NHWD)", "lang": "en"}, {"value": "Entsorgter nicht gefährlicher Abfall (NHWD)", "lang": "de"}], "type": "flow data set", "refObjectId": "b29ef66b-e286-4afa-949f-62f1a7b4d7fa", "uri": "../flows/b29ef66b-e286-4afa-949f-62f1a7b4d7fa.xml"}, "exchange direction": "OUTPUT", "other": {"anies": [{"name": "referenceToUnitGroupDataSet", "value": {"shortDescription": [{"value": "kg", "lang": "en"}], "type": "unit group data set", "refObjectId": "ad38d542-3fe9-439d-9b95-2f5f7752acaf", "uri": "../unitgroups/ad38d542-3fe9-439d-9b95-2f5f7752acaf.xml"}}, {"value": "7.85", "module": "A1-A3"}, {"value": "0.00477", "module": "A4"}, {"value": "0.137", "module": "A5"}, {"value": "4.96", "module": "B6"}, {"value": "5.23E-05", "module": "C1"}, {"value": "0.000483", "module": "C2"}, {"value": "1.04", "module": "C3"}, {"value": "0", "module": "C4"}, {"value": "-4.87", "module": "D"}]}, "resolvedFlowVersion": "38.00.000", "flowProperties": [], "typeOfFlow": "Other flow", "classification": {"classHierarchy": "Quantities / Environmental quantities / EPD EN 15804 / LCI indicators", "name": "GaBiCategories"}}, {"dataSetInternalID": 13, "referenceToFlowDataSet": {"shortDescription": [{"value": "Radioactive waste disposed (RWD)", "lang": "en"}, {"value": "Entsorgter radioaktiver Abfall (RWD)", "lang": "de"}], "type": "flow data set", "refObjectId": "3449546e-52ad-4b39-b809-9fb77cea8ff6", "uri": "../flows/3449546e-52ad-4b39-b809-9fb77cea8ff6.xml"}, "exchange direction": "OUTPUT", "other": {"anies": [{"name": "referenceToUnitGroupDataSet", "value": {"shortDescription": [{"value": "kg", "lang": "en"}], "type": "unit group data set", "refObjectId": "ad38d542-3fe9-439d-9b95-2f5f7752acaf", "uri": "../unitgroups/ad38d542-3fe9-439d-9b95-2f5f7752acaf.xml"}}, {"value": "0.0474", "module": "A1-A3"}, {"value": "4.29E-05", "module": "A4"}, {"value": "0.000235", "module": "A5"}, {"value": "1.06", "module": "B6"}, {"value": "1.12E-05", "module": "C1"}, {"value": "4.93E-06", "module": "C2"}, {"value": "0.000145", "module": "C3"}, {"value": "0", "module": "C4"}, {"value": "-0.0241", "module": "D"}]}, "resolvedFlowVersion": "38.00.000", "flowProperties": [], "typeOfFlow": "Other flow", "classification": {"classHierarchy": "Quantities / Environmental quantities / EPD EN 15804 / LCI indicators", "name": "GaBiCategories"}}, {"dataSetInternalID": 14, "referenceToFlowDataSet": {"shortDescription": [{"value": "Components for re-use (CRU)", "lang": "en"}, {"value": "Komponenten für die Wiederverwendung (CRU)", "lang": "de"}], "type": "flow data set", "refObjectId": "a2b32f97-3fc7-4af2-b209-525bc6426f33", "uri": "../flows/a2b32f97-3fc7-4af2-b209-525bc6426f33.xml"}, "exchange direction": "OUTPUT", "other": {"anies": [{"name": "referenceToUnitGroupDataSet", "value": {"shortDescription": [{"value": "kg", "lang": "en"}], "type": "unit group data set", "refObjectId": "ad38d542-3fe9-439d-9b95-2f5f7752acaf", "uri": "../unitgroups/ad38d542-3fe9-439d-9b95-2f5f7752acaf.xml"}}, {"value": "0", "module": "A1-A3"}, {"value": "0", "module": "A4"}, {"value": "0", "module": "A5"}, {"value": "0", "module": "B6"}, {"value": "0", "module": "C1"}, {"value": "0", "module": "C2"}, {"value": "0", "module": "C3"}, {"value": "0", "module": "C4"}, {"value": "0", "module": "D"}]}, "resolvedFlowVersion": "38.00.000", "flowProperties": [], "typeOfFlow": "Other flow", "classification": {"classHierarchy": "Quantities / Environmental quantities / EPD EN 15804 / LCI indicators", "name": "GaBiCategories"}}, {"dataSetInternalID": 15, "referenceToFlowDataSet": {"shortDescription": [{"value": "Materials for recycling (MFR)", "lang": "en"}, {"value": "Stoffe zum Recycling (MFR)", "lang": "de"}], "type": "flow data set", "refObjectId": "d7fe48a5-4103-49c8-9aae-b0b5dfdbd6ae", "uri": "../flows/d7fe48a5-4103-49c8-9aae-b0b5dfdbd6ae.xml"}, "exchange direction": "OUTPUT", "other": {"anies": [{"name": "referenceToUnitGroupDataSet", "value": {"shortDescription": [{"value": "kg", "lang": "en"}], "type": "unit group data set", "refObjectId": "ad38d542-3fe9-439d-9b95-2f5f7752acaf", "uri": "../unitgroups/ad38d542-3fe9-439d-9b95-2f5f7752acaf.xml"}}, {"value": "2.89348", "module": "A1-A3"}, {"value": "0", "module": "A4"}, {"value": "0", "module": "A5"}, {"value": "0", "module": "B6"}, {"value": "0", "module": "C1"}, {"value": "0", "module": "C2"}, {"value": "21.153685", "module": "C3"}, {"value": "0", "module": "C4"}, {"value": "0", "module": "D"}]}, "resolvedFlowVersion": "38.00.000", "flowProperties": [], "typeOfFlow": "Other flow", "classification": {"classHierarchy": "Quantities / Environmental quantities / EPD EN 15804 / LCI indicators", "name": "GaBiCategories"}}, {"dataSetInternalID": 16, "referenceToFlowDataSet": {"shortDescription": [{"value": "Materials for energy recovery (MER)", "lang": "en"}, {"value": "Stoffe für die Energierückgewinnung (MER)", "lang": "de"}], "type": "flow data set", "refObjectId": "59a9181c-3aaf-46ee-8b13-2b3723b6e447", "uri": "../flows/59a9181c-3aaf-46ee-8b13-2b3723b6e447.xml"}, "exchange direction": "OUTPUT", "other": {"anies": [{"name": "referenceToUnitGroupDataSet", "value": {"shortDescription": [{"value": "kg", "lang": "en"}], "type": "unit group data set", "refObjectId": "ad38d542-3fe9-439d-9b95-2f5f7752acaf", "uri": "../unitgroups/ad38d542-3fe9-439d-9b95-2f5f7752acaf.xml"}}, {"value": "0", "module": "A1-A3"}, {"value": "0", "module": "A4"}, {"value": "2.9808", "module": "A5"}, {"value": "0", "module": "B6"}, {"value": "0", "module": "C1"}, {"value": "0", "module": "C2"}, {"value": "3.42727", "module": "C3"}, {"value": "0", "module": "C4"}, {"value": "0", "module": "D"}]}, "resolvedFlowVersion": "38.00.000", "flowProperties": [], "typeOfFlow": "Other flow", "classification": {"classHierarchy": "Quantities / Environmental quantities / EPD EN 15804 / LCI indicators", "name": "GaBiCategories"}}, {"dataSetInternalID": 17, "referenceToFlowDataSet": {"shortDescription": [{"value": "Exported electrical energy (EEE)", "lang": "en"}, {"value": "Exportierte elektrische Energie (EEE)", "lang": "de"}], "type": "flow data set", "refObjectId": "4da0c987-2b76-40d6-9e9e-82a017aaaf29", "uri": "../flows/4da0c987-2b76-40d6-9e9e-82a017aaaf29.xml"}, "exchange direction": "OUTPUT", "other": {"anies": [{"name": "referenceToUnitGroupDataSet", "value": {"shortDescription": [{"value": "MJ", "lang": "en"}], "type": "unit group data set", "refObjectId": "93a60a57-a3c8-11da-a746-0800200c9a66", "uri": "../unitgroups/93a60a57-a3c8-11da-a746-0800200c9a66.xml"}}, {"value": "0", "module": "A1-A3"}, {"value": "0", "module": "A4"}, {"value": "6.57226", "module": "A5"}, {"value": "0", "module": "B6"}, {"value": "0", "module": "C1"}, {"value": "0", "module": "C2"}, {"value": "12.929", "module": "C3"}, {"value": "0", "module": "C4"}, {"value": "0", "module": "D"}]}, "resolvedFlowVersion": "38.00.000", "flowProperties": [], "typeOfFlow": "Other flow", "classification": {"classHierarchy": "Quantities / Environmental quantities / EPD EN 15804 / LCI indicators", "name": "GaBiCategories"}}, {"dataSetInternalID": 18, "referenceToFlowDataSet": {"shortDescription": [{"value": "Exported thermal energy (EET)", "lang": "en"}, {"value": "Exportierte thermische Energie (EET)", "lang": "de"}], "type": "flow data set", "refObjectId": "98daf38a-7a79-46d3-9a37-2b7bd0955810", "uri": "../flows/98daf38a-7a79-46d3-9a37-2b7bd0955810.xml"}, "exchange direction": "OUTPUT", "other": {"anies": [{"name": "referenceToUnitGroupDataSet", "value": {"shortDescription": [{"value": "MJ", "lang": "en"}], "type": "unit group data set", "refObjectId": "93a60a57-a3c8-11da-a746-0800200c9a66", "uri": "../unitgroups/93a60a57-a3c8-11da-a746-0800200c9a66.xml"}}, {"value": "0", "module": "A1-A3"}, {"value": "0", "module": "A4"}, {"value": "11.91265", "module": "A5"}, {"value": "0", "module": "B6"}, {"value": "0", "module": "C1"}, {"value": "0", "module": "C2"}, {"value": "27.593", "module": "C3"}, {"value": "0", "module": "C4"}, {"value": "0", "module": "D"}]}, "resolvedFlowVersion": "38.00.000", "flowProperties": [], "typeOfFlow": "Other flow", "classification": {"classHierarchy": "Quantities / Environmental quantities / EPD EN 15804 / LCI indicators", "name": "GaBiCategories"}}]}, "LCIAResults": {"LCIAResult": [{"referenceToLCIAMethodDataSet": {"shortDescription": [{"value": "Global warming potential (GWP)", "lang": "en"}, {"value": "Globales Erwärmungspotenzial (GWP)", "lang": "de"}], "type": "LCIA method data set", "refObjectId": "77e416eb-a363-4258-a04e-171d843a6460", "uri": "../lciamethods/77e416eb-a363-4258-a04e-171d843a6460.xml"}, "other": {"anies": [{"name": "referenceToUnitGroupDataSet", "value": {"shortDescription": [{"value": "kg CO_(2) eq", "lang": "en"}], "type": "unit group data set", "refObjectId": "1ebf3012-d0db-4de2-aefd-ef30cedb0be1", "uri": "../unitgroups/1ebf3012-d0db-4de2-aefd-ef30cedb0be1.xml"}}, {"value": "207", "module": "A1-A3"}, {"value": "2.77", "module": "A4"}, {"value": "4.8", "module": "A5"}, {"value": "390", "module": "B6"}, {"value": "0.00411", "module": "C1"}, {"value": "0.214", "module": "C2"}, {"value": "6.73", "module": "C3"}, {"value": "0", "module": "C4"}, {"value": "-30.4", "module": "D"}]}}, {"referenceToLCIAMethodDataSet": {"shortDescription": [{"value": "Depletion potential of the stratospheric ozone layer (ODP)", "lang": "en"}, {"value": "Abbau Potential der stratosphärischen Ozonschicht (ODP)", "lang": "de"}], "type": "LCIA method data set", "refObjectId": "06dcd26f-025f-401a-a7c1-5e457eb54637", "uri": "../lciamethods/06dcd26f-025f-401a-a7c1-5e457eb54637.xml"}, "other": {"anies": [{"name": "referenceToUnitGroupDataSet", "value": {"shortDescription": [{"value": "kg CFC11 eq", "lang": "en"}], "type": "unit group data set", "refObjectId": "88054749-b0a6-47ea-a82b-dc5b29326512", "uri": "../unitgroups/88054749-b0a6-47ea-a82b-dc5b29326512.xml"}}, {"value": "1.12E-05", "module": "A1-A3"}, {"value": "4.1E-16", "module": "A4"}, {"value": "4.44E-15", "module": "A5"}, {"value": "1.17E-11", "module": "B6"}, {"value": "1.23E-16", "module": "C1"}, {"value": "6.81E-17", "module": "C2"}, {"value": "4.19E-14", "module": "C3"}, {"value": "0", "module": "C4"}, {"value": "-1.27E-13", "module": "D"}]}}, {"referenceToLCIAMethodDataSet": {"shortDescription": [{"value": "Acidification potential of land and water (AP)", "lang": "en"}, {"value": "Versauerungspotenzial von Boden und Wasser (AP)", "lang": "de"}], "type": "LCIA method data set", "refObjectId": "b4274add-93b7-4905-a5e4-2e878c4e4216", "uri": "../lciamethods/b4274add-93b7-4905-a5e4-2e878c4e4216.xml"}, "other": {"anies": [{"name": "referenceToUnitGroupDataSet", "value": {"shortDescription": [{"value": "kg SO_(2) eq", "lang": "en"}], "type": "unit group data set", "refObjectId": "bc50c624-a9bc-45b1-a9b0-e6b10d00476f", "uri": "../unitgroups/bc50c624-a9bc-45b1-a9b0-e6b10d00476f.xml"}}, {"value": "1.16", "module": "A1-A3"}, {"value": "0.0434", "module": "A4"}, {"value": "0.00187", "module": "A5"}, {"value": "0.819", "module": "B6"}, {"value": "8.63E-06", "module": "C1"}, {"value": "0.00091", "module": "C2"}, {"value": "0.0022", "module": "C3"}, {"value": "0", "module": "C4"}, {"value": "-0.108", "module": "D"}]}}, {"referenceToLCIAMethodDataSet": {"shortDescription": [{"value": "Eutrophication potential (EP)", "lang": "en"}, {"value": "Eutrophierungspotenzial (EP)", "lang": "de"}], "type": "LCIA method data set", "refObjectId": "f58827d0-b407-4ec6-be75-8b69efb98a0f", "uri": "../lciamethods/f58827d0-b407-4ec6-be75-8b69efb98a0f.xml"}, "other": {"anies": [{"name": "referenceToUnitGroupDataSet", "value": {"shortDescription": [{"value": "kg PO_(4)^(3) eq", "lang": "en"}], "type": "unit group data set", "refObjectId": "67b5401d-873c-485f-bcf3-6ae83b918822", "uri": "../unitgroups/67b5401d-873c-485f-bcf3-6ae83b918822.xml"}}, {"value": "0.639", "module": "A1-A3"}, {"value": "0.00574", "module": "A4"}, {"value": "0.000295", "module": "A5"}, {"value": "0.0906", "module": "B6"}, {"value": "9.55E-07", "module": "C1"}, {"value": "0.000227", "module": "C2"}, {"value": "0.000228", "module": "C3"}, {"value": "0", "module": "C4"}, {"value": "-0.006", "module": "D"}]}}, {"referenceToLCIAMethodDataSet": {"shortDescription": [{"value": "Formation potential of tropospheric ozone photochemical oxidants (POCP)", "lang": "en"}, {"value": "Bildungspotential für troposphärisches Ozon (POCP)", "lang": "de"}], "type": "LCIA method data set", "refObjectId": "1e84a202-dae6-42aa-9e9d-71ea48b8be00", "uri": "../lciamethods/1e84a202-dae6-42aa-9e9d-71ea48b8be00.xml"}, "other": {"anies": [{"name": "referenceToUnitGroupDataSet", "value": {"shortDescription": [{"value": "kg Ethen eq", "lang": "en"}], "type": "unit group data set", "refObjectId": "01c26c17-9a76-406e-8295-f17b55fd909e", "uri": "../unitgroups/01c26c17-9a76-406e-8295-f17b55fd909e.xml"}}, {"value": "0.0801", "module": "A1-A3"}, {"value": "-0.000725", "module": "A4"}, {"value": "0.000146", "module": "A5"}, {"value": "0.0583", "module": "B6"}, {"value": "6.15E-07", "module": "C1"}, {"value": "-0.000343", "module": "C2"}, {"value": "8.85E-05", "module": "C3"}, {"value": "0", "module": "C4"}, {"value": "-0.00956", "module": "D"}]}}, {"referenceToLCIAMethodDataSet": {"shortDescription": [{"value": "Abiotic depletion potential for non fossil resources (ADPE)", "lang": "en"}, {"value": "Potenzial für den abiotischen Abbau nicht fossiler Ressourcen (ADPE)", "lang": "de"}], "type": "LCIA method data set", "refObjectId": "f7c73bb9-ab1a-4249-9c6d-379a0de6f67e", "uri": "../lciamethods/f7c73bb9-ab1a-4249-9c6d-379a0de6f67e.xml"}, "other": {"anies": [{"name": "referenceToUnitGroupDataSet", "value": {"shortDescription": [{"value": "kg Sb eq", "lang": "en"}], "type": "unit group data set", "refObjectId": "54ccd2d9-a32a-4fc2-923d-f2c8c93e89d4", "uri": "../unitgroups/54ccd2d9-a32a-4fc2-923d-f2c8c93e89d4.xml"}}, {"value": "0.0558", "module": "A1-A3"}, {"value": "1.61E-07", "module": "A4"}, {"value": "1.71E-05", "module": "A5"}, {"value": "0.00013", "module": "B6"}, {"value": "1.37E-09", "module": "C1"}, {"value": "2.01E-08", "module": "C2"}, {"value": "9.89E-07", "module": "C3"}, {"value": "0", "module": "C4"}, {"value": "-0.00309", "module": "D"}]}}, {"referenceToLCIAMethodDataSet": {"shortDescription": [{"value": "Abiotic depletion potential for fossil resources (ADPF)", "lang": "en"}, {"value": "Potenzial für den abiotischen Abbau fossiler Brennstoffe (ADPF)", "lang": "de"}], "type": "LCIA method data set", "refObjectId": "804ebcdf-309d-4098-8ed8-fdaf2f389981", "uri": "../lciamethods/804ebcdf-309d-4098-8ed8-fdaf2f389981.xml"}, "other": {"anies": [{"name": "referenceToUnitGroupDataSet", "value": {"shortDescription": [{"value": "MJ", "lang": "en"}], "type": "unit group data set", "refObjectId": "93a60a57-a3c8-11da-a746-0800200c9a66", "uri": "../unitgroups/93a60a57-a3c8-11da-a746-0800200c9a66.xml"}}, {"value": "2650", "module": "A1-A3"}, {"value": "36.1", "module": "A4"}, {"value": "7.29", "module": "A5"}, {"value": "4320", "module": "B6"}, {"value": "0.0456", "module": "C1"}, {"value": "2.92", "module": "C2"}, {"value": "3.77", "module": "C3"}, {"value": "0", "module": "C4"}, {"value": "-341", "module": "D"}]}}]}, "otherAttributes": {"{http://www.indata.network/EPD/2019}epd-version": "1.2"}, "version": "1.1", "locations": "../ILCDLocations.xml"}