{"processInformation": {"dataSetInformation": {"UUID": "64318385-991b-4aec-83a4-99c59f6f2471", "name": {"baseName": [{"value": "Bachl ReXPS - Extruded Polystyrene (XPS) foam board", "lang": "de"}, {"value": "Bachl ReXPS - Extruded Polystyrene (XPS) foam board", "lang": "en"}], "functionalUnitFlowProperties": [{"lang": "de"}]}, "classificationInformation": {"classification": [{"class": [{"value": "Dämmstoffe", "level": 0, "classId": "2"}, {"value": "Extrudiertes Polystyrol (XPS)", "level": 1, "classId": "2.3"}, {"value": "XPS weiß", "level": 2, "classId": "2.3.01"}], "name": "OEKOBAU.DAT"}, {"class": [{"value": "02 Bauprodukte", "level": 0}, {"value": "Wärmedämmungsprodukte", "level": 1}, {"value": "Dämmstoffe aus Schaumkunststoffen", "level": 2}], "name": "IBUCategories"}]}, "generalComment": [{"value": "Bachl ReXPS ist ein Polystyrol-Extruderschaumstoff (XPS) aus 100 % wiedergewonnenem und recyceltem Polystyrol, der nach EN 13164 gefertigt wird und in Plattenform mit Dichten zwischen 30 und 35 kg/m erhltlich ist. Bachl ReXPS-Dmmplatten werden im Verband versetzt oder stumpf gestoen. Die EPD gilt nur fr das unbeschichtete Produkt; eine Beschichtung und weitere Produktbehandlungen werden nicht bercksichtigt.\n\nFr das Inverkehrbringen des Produkts in der EU/EFTA (mit Ausnahme der Schweiz) gilt die Verordnung (EU) Nr. 305/2011 (CPR). Das Produkt bentigt eine Leistungserklrung unter Bercksichtigung der EN 13164:2012 und A1:2015 – Wrmedmmstoffe fr Gebude  Werkmig hergestellte Produkte aus extrudiertem Polystyrolschaum (XPS)  Spezifikation und die CE-Kennzeichnung. Fr die Anwendung und Nutzung gelten die jeweiligen nationalen Bestimmungen.", "lang": "de"}, {"value": "Bachl ReXPS is an extruded polystyrene foam (XPS) made of 100% recycled and reclaimed polystyrene, manufactured according to EN 13164 and available in sheet form with a density range of 30-35 kg/m. Bachl ReXPS panels are supplied with a butt edge or shiplap. The EPD only applies to an unlaminated product; Lamination and additional product treatment are not taken into account. \nRegulation (EU) No. 305/2011 (CPR) applies to placing the product on the market in the European Union/European Free Trade Association (EU/EFTA) (with the exception of Switzerland). The Product requires a declaration of performance taking into account EN 13164:2012+A1:2015 Thermal insulation products for buildings - Factory made extruded polystyrene foam (XPS) products - Specification and CE marking. The respective national regulations apply to application and use.", "lang": "en"}], "other": {"anies": [{"scenario": [{"description": [{"value": "Zur Energierückgewinnung", "lang": "de"}, {"value": "100% incineration", "lang": "en"}], "name": "S1", "default": true}, {"description": [{"value": "Recycling", "lang": "de"}, {"value": "100% recycling", "lang": "en"}], "name": "S2"}, {"description": [{"value": "Deponierung", "lang": "de"}, {"value": "100% landfill", "lang": "en"}], "name": "S3"}]}]}}, "quantitativeReference": {"referenceToReferenceFlow": [0]}, "time": {"referenceYear": 2022, "dataSetValidUntil": 2027, "other": {"anies": [{"name": "publicationDateOfEPD", "value": 1669766400000}]}}, "geography": {"locationOfOperationSupplyOrProduction": {"location": "RER"}}, "technology": {"technologyDescriptionAndIncludedProcesses": [{"value": "Bachl ReXPS ist ein Polystyrol-Extruderschaumstoff (XPS) aus 100 % wiedergewonnenem und recyceltem Polystyrol, der nach EN 13164 gefertigt wird und in Plattenform mit Dichten zwischen 30 und 35 kg/m³ erhältlich ist. Bachl ReXPSDämmplatten werden im Verband versetzt oder stumpf gestoßen. Die EPD gilt nur für das unbeschichtete Produkt; eine Beschichtung und weitere Produktbehandlungen werden nicht berücksichtigt. \nTechnische Daten: \nSchallabsorptionskoeffizient und dynamische Steifigkeit sind fr Bachl ReXPS nicht relevant, da diese Dmmplatten nicht zur Verbesserung der Raumakustik oder Beeinflussung der Schalldmmung eingesetzt werden. \n\nBezglich des Brandverhaltens gengen diese Produkte der Brandschutzklasse E nach EN 13501-1 (auer fr Skandinavien). \nDeklarierte Einheit: \nDie deklarierte Einheit ist 1 m3 der ReXPS-Dmmplatte. Die Dichte des Produktes betrgt 32,7 kg/m.", "lang": "de"}, {"value": "Bachl ReXPS is an extruded polystyrene foam (XPS) made of 100% recycled and reclaimed polystyrene, manufactured according to EN 13164 and available in sheet form with a density range of 30-35 kg/m³. Bachl ReXPS panels are supplied with a butt edge or shiplap. The EPD only applies to an unlaminated product; Lamination and additional product treatment are not taken into account. \nTechnical data: \nSound absorption coefficient and dynamic rigidity are not relevant for Bachl ReXPS because this insulation panel is not used to improve room acoustics or impact sound insulation. For fire performance, these products except in Scandinavia achieve the fire classification Euroclass E according to EN 13501-1. \nDeclared unit: \nThe declared unit is 1 m3 of the Re-XPS insulation board. The density of the product is 32.7 kg/m.", "lang": "en"}], "technologicalApplicability": [{"value": "Dank der vielfltigen Leistungsmerkmale von Bachl ReXPS eignet sich der Werkstoff fr zahlreiche Anwendungen, wie zur Perimeterdmmung, zur Bodendmmung einschlielich der Dmmung hochbelasteter Industriebden, zur Wrmebrckendmmung an Auenwnden, zur Kerndmmung, Deckendmmung in landwirtschaftlich genutzten Gebuden, fr Fertigelemente, z. B. Verbundplatten.", "lang": "de"}, {"value": "The variety of the performance properties of Bachl ReXPS make it suitable for use in a large number of applications such as: perimeter insulation, floor insulation including insulation of highly loaded industrial floors, insulation of thermal bridges for exterior walls, insulation of cavity walls, agricultural building ceiling insulation, prefabricated elements e.g. building sandwich panels.", "lang": "en"}]}}, "modellingAndValidation": {"LCIMethodAndAllocation": {"typeOfDataSet": "EPD", "referenceToLCAMethodDetails": [{"shortDescription": [{"value": "Dämmstoffe aus Schaumkunststoffen.pdf", "lang": "de"}], "type": "source data set", "refObjectId": "e95d0a4a-325b-4d41-ac7a-42965593e5b2"}], "other": {"anies": [{"name": "subType", "value": "specific dataset"}]}}, "dataSourcesTreatmentAndRepresentativeness": {"referenceToDataSource": [{"shortDescription": [{"value": "GaBi Database (all versions)", "lang": "de"}], "type": "source data set", "refObjectId": "28d74cc0-db8b-4d7e-bc44-5f6d56ce0c4a"}, {"shortDescription": [{"value": "GaBi Database Edition 2022, CUP 2022.01", "lang": "de"}], "type": "source data set", "refObjectId": "86f664e2-7dab-4722-aad7-4c5206a4123b"}], "useAdviceForDataSet": [{"value": "Gültigkeitsbereich: \nDie Daten wurden von einem Produktionsstandort in Tittling, Deutschland, fr das Jahr 2021 bereitgestellt. \nSystemgrenze: \nTyp der EPD nach EN 15804: Wiege bis Werkstor  mit Optionen, Module C1C4 und D. Die folgenden Module werden deklariert: A1A3, C, D und zustzliche Module: A4 + A5.  \n\nProduktion  Module A1A3 \nDas Produktionsstadium umfasst:\nRohstoffbereitstellung (A1): extern recyceltes Polystyrol-Regranulat, Polystyrol-Briketts und ihr Recycling-Prozess vor Ort, Treibmittel, Co-Treibmittel und Flammschutzmittel.\nTransport zum Hersteller (A2)\nHerstellung (A3) einschlielich Bereitstellung aller Rohstoffe, Produkte und Energien sowie Abfallaufbereitung bis zum Ende der Abfalleigenschaft.\nStadium der Errichtung des Bauwerks  Module A4A5\nDas Stadium der Errichtung des Bauwerks umfasst:\nTransport zur Baustelle (A4)\nAufbereitung des Verpackungsmaterials (A5); Gutschriften fr potenziell durch die Substitution von Elektro- und Wrmeenergie vermiedene Lasten werden in Modul D deklariert. \n\nEntsorgungsstadium  Module C1C4 und D \nDas Entsorgungsstadium umfasst:\n\nManueller Rckbau (C1)\nTransport zur Entsorgung (C2)\nAbfallbehandlung und -beseitigung (C) mit drei 100-%-Szenarien (Szenario 1: thermische Aufbereitung (C3/1); Szenario 2: Recycling (C3/2); Szenario 3: Deponie (C4/3))\nWiederverwendungs-, Rckgewinnungs- oder Recyclingpotenzial Im Modul D wurden keine Gutschriften aus Szenarien aus dem Entsorgungsstadium (C3/1, C3/2 oder C4/3) bercksichtigt. Die Gutschriften unter D/1, D/2 und D/3 bercksichtigen ausschlielich die vermiedenen Lasten, die ber die Umkehrung des Stromnetzmixes und der Wrmeenergie aus Erdgas bei der Verpackungsaufbereitung (A5) berechnet wurden.", "lang": "de"}, {"value": "Scope: \nThe data have been provided by one production site based in Tittling, Germany for the year 2021. \nSystem boundary: \nType of EPD according to EN 15804: \"cradle to gate with options, modules C1–C4, and module D\". The following modules are declared: A1–A3, C, D and additional modules: A4 + A5. \n\nProduction - Modules A1-A3\nThe product stage includes:\n\nRaw material supply (A1): polystyrene (PS) re-granulates recycled externally, polystyrene (PS) briquettes and their recycling process on-site, blowing agents, co-blowing agents, and flame retardants.\nTransport to the manufacturer (A2) \nManufacturing (A3), including provision of all materials, products and energy, as well as waste processing up to the end-of-waste state.Construction stage - Modules A4-A5\nThe construction process stage includes:\n\nTransport to the construction site (A4)\n\nTreatment of packaging material (A5) credits for potential avoided burdens due to energy substitution of electricity and thermal energy generation are declared in module D.\nEnd-of-life stage– Modules C1-C4 and D\n\nThe end-of-life stage includes\nManual dismantling (C1)\nTransport to EoL (C2) \nWaste processing & disposal (C) with three 100 % scenarios (scenario 1: thermal treatment (C3/1); scenario 2: Recycling (C3/2); scenario 3: landfill (C4/3))\nReuse, recovery or recycling potential (D) - beyond system boundary. No credits were accounted from any of the EoL scenarios (C3/1, C3/2, or C4/3) in module D. The credits in D/1, D/2, and D/3 are solely\naccounting for the avoided burdens calculated by the inversion of electricity grid mix and thermal energy from natural gas during packaging treatment (A5).", "lang": "en"}], "other": {"anies": [{"name": "referenceToOriginalEPD", "value": {"shortDescription": {"value": "Bachl ReXPS - Extruded Polystyrene (XPS) foam board.pdf", "defaultValue": "Bachl ReXPS - Extruded Polystyrene (XPS) foam board.pdf", "lstrings": [{"lang": "de", "value": "Bachl ReXPS - Extruded Polystyrene (XPS) foam board.pdf"}]}, "type": "source data set", "uuid": {"uuid": "88c0091e-ce99-4d3f-85e7-286a5f0cffe4"}, "refObjectId": "88c0091e-ce99-4d3f-85e7-286a5f0cffe4", "resourceURLs": ["https://oekobaudat.de/OEKOBAU.DAT/resource/sources/88c0091e-ce99-4d3f-85e7-286a5f0cffe4/Bachl_ReXPS_-_Extruded_Polystyrene_XPS_foam_board_18590.pdf?version=00.02.000"]}}]}}, "validation": {"review": [{"referenceToNameOfReviewerAndInstitution": [{"shortDescription": [{"value": "Institut Bauen und Umwelt e. V.", "lang": "de"}], "type": "contact data set", "refObjectId": "d111dbec-b024-4be5-86c5-752d6eb2cf95", "uri": "../contacts/d111dbec-b024-4be5-86c5-752d6eb2cf95.xml"}], "type": "Accredited third party review"}]}, "complianceDeclarations": {"compliance": [{"referenceToComplianceSystem": {"shortDescription": [{"value": "DIN EN 15804+A2", "lang": "de"}], "type": "source data set", "refObjectId": "c0016b33-8cf7-415c-ac6e-deba0d21440d", "uri": "../sources/c0016b33-8cf7-415c-ac6e-deba0d21440d.xml"}}, {"referenceToComplianceSystem": {"shortDescription": [{"value": "ISO 14025", "lang": "de"}], "type": "source data set", "refObjectId": "4f2eb655-6e44-4874-a95a-e28f5442cd4d", "uri": "../sources/4f2eb655-6e44-4874-a95a-e28f5442cd4d.xml"}}]}}, "administrativeInformation": {"commissionerAndGoal": {"referenceToCommissioner": [{"shortDescription": [{"value": "Karl Bachl Kunststoffverarbeitung GmbH & Co. KG", "lang": "de"}], "type": "contact data set", "refObjectId": "14474393-68b0-40e4-b480-5346378d4751", "uri": "../contacts/14474393-68b0-40e4-b480-5346378d4751.xml"}]}, "dataGenerator": {"referenceToPersonOrEntityGeneratingTheDataSet": [{"shortDescription": [{"value": "Sphera Solutions GmbH", "lang": "de"}], "type": "contact data set", "refObjectId": "623edf96-39d1-4e6f-9892-674c7228546b", "uri": "../contacts/623edf96-39d1-4e6f-9892-674c7228546b.xml"}]}, "dataEntryBy": {"timeStamp": 1669766400000, "referenceToDataSetFormat": [{"shortDescription": [{"value": "ILCD Format", "lang": "de"}], "type": "source data set", "refObjectId": "a97a0155-0234-4b87-b4ce-a45da52f2a40", "uri": "../sources/a97a0155-0234-4b87-b4ce-a45da52f2a40.xml"}, {"shortDescription": [{"value": "EPD-Datenformaterweiterungen v1.2", "lang": "de"}, {"value": "EPD Data Format Extensions v1.2", "lang": "en"}], "type": "source data set", "refObjectId": "a29449fd-aa2f-4de8-b5d7-4b06b43c6fde", "uri": "../sources/a29449fd-aa2f-4de8-b5d7-4b06b43c6fde.xml"}]}, "publicationAndOwnership": {"dataSetVersion": "00.10.000", "referenceToRegistrationAuthority": {"shortDescription": [{"value": "Institut Bauen und Umwelt e. V.", "lang": "de"}], "type": "contact data set", "refObjectId": "d111dbec-b024-4be5-86c5-752d6eb2cf95", "uri": "../contacts/d111dbec-b024-4be5-86c5-752d6eb2cf95.xml"}, "registrationNumber": "EPD-BAC-20220231-CBA2-DE", "referenceToOwnershipOfDataSet": {"shortDescription": [{"value": "Karl Bachl Kunststoffverarbeitung GmbH & Co. KG", "lang": "de"}], "type": "contact data set", "refObjectId": "14474393-68b0-40e4-b480-5346378d4751", "uri": "../contacts/14474393-68b0-40e4-b480-5346378d4751.xml"}, "copyright": true, "licenseType": "Free of charge for all users and uses", "accessRestrictions": [{"value": "None", "lang": "en"}], "other": {"anies": [{"name": "referenceToPublisher", "value": {"shortDescription": [{"value": "Institut Bauen und Umwelt e. V.", "lang": "de"}], "type": "contact data set", "refObjectId": "d111dbec-b024-4be5-86c5-752d6eb2cf95", "uri": "../contacts/d111dbec-b024-4be5-86c5-752d6eb2cf95.xml"}}]}}}, "exchanges": {"exchange": [{"dataSetInternalID": 0, "referenceToFlowDataSet": {"shortDescription": [{"value": "Bachl ReXPS - Extrudierte Polystyrol-Schaumstoffplatten (Bachl ReXPS - Extrudierte Polystyrol-Schaumstoffplatten)", "lang": "de"}], "type": "flow data set", "refObjectId": "abe7d9a9-fab6-36f9-1c63-db370696387b", "uri": "../flows/abe7d9a9-fab6-36f9-1c63-db370696387b.xml"}, "meanAmount": 1.0, "referencesToDataSource": {}, "referenceFlow": true, "resolvedFlowVersion": "00.02.000", "resultingflowAmount": 1.0, "flowProperties": [{"name": [{"lang": "en", "value": "Volume"}, {"lang": "de", "value": "Volumen"}], "uuid": "93a60a56-a3c8-22da-a746-0800200c9a66", "referenceFlowProperty": true, "meanValue": 1.0, "referenceUnit": "m3", "unitGroupUUID": "cd950537-0a98-4044-9ba7-9f9a68d0a504"}], "materialProperties": [{"name": "gross density", "value": "32.7", "unit": "kg/m^3", "unitDescription": "kilograms per cubic metre"}], "typeOfFlow": "Product flow", "classification": {"classHierarchy": "Dämmstoffe / Extrudiertes Polystyrol (XPS) / XPS weiß", "name": "OEKOBAU.DAT"}}, {"dataSetInternalID": 1, "referenceToFlowDataSet": {"shortDescription": [{"value": "Erneuerbare Primärenergie als Energieträger (PERE)", "lang": "de"}, {"value": "Renewable primary energy as energy carrier (PERE)", "lang": "en"}], "type": "flow data set", "refObjectId": "20f32be5-0398-4288-9b6d-accddd195317", "uri": "../flows/20f32be5-0398-4288-9b6d-accddd195317.xml"}, "exchange direction": "INPUT", "other": {"anies": [{"name": "referenceToUnitGroupDataSet", "value": {"shortDescription": [{"value": "MJ", "lang": "de"}], "type": "unit group data set", "refObjectId": "93a60a57-a3c8-11da-a746-0800200c9a66", "uri": "../unitgroups/93a60a57-a3c8-11da-a746-0800200c9a66.xml"}}, {"value": "69.3662340570049", "module": "A1-A3"}, {"value": "0.380564697823308", "module": "A4"}, {"value": "0.057320858356698", "module": "A5"}, {"value": "0", "module": "C1"}, {"value": "0.371853989685717", "module": "C2"}, {"value": "2.91095340873227", "module": "C3", "scenario": "S1"}, {"value": "47.1481094156143", "module": "C3", "scenario": "S2"}, {"value": "2.70343471790903", "module": "C4"}, {"value": "-4.62137284150507", "module": "D", "scenario": "S1"}, {"value": "-4.62137284150507", "module": "D", "scenario": "S2"}, {"value": "-4.62137284150507", "module": "D", "scenario": "S3"}]}, "resolvedFlowVersion": "38.00.000", "flowProperties": [], "typeOfFlow": "Other flow", "classification": {"classHierarchy": "Quantities", "name": "GaBiCategories"}}, {"dataSetInternalID": 2, "referenceToFlowDataSet": {"shortDescription": [{"value": "Erneuerbare Primärenergie zur stofflichen Nutzung (PERM)", "lang": "de"}, {"value": "Renewable primary energy resources as material utilization (PERM)", "lang": "en"}], "type": "flow data set", "refObjectId": "fb3ec0de-548d-4508-aea5-00b73bf6f702", "uri": "../flows/fb3ec0de-548d-4508-aea5-00b73bf6f702.xml"}, "exchange direction": "INPUT", "other": {"anies": [{"name": "referenceToUnitGroupDataSet", "value": {"shortDescription": [{"value": "MJ", "lang": "de"}], "type": "unit group data set", "refObjectId": "93a60a57-a3c8-11da-a746-0800200c9a66", "uri": "../unitgroups/93a60a57-a3c8-11da-a746-0800200c9a66.xml"}}, {"value": "0", "module": "A1-A3"}, {"value": "0", "module": "A4"}, {"value": "0", "module": "A5"}, {"value": "0", "module": "C1"}, {"value": "0", "module": "C2"}, {"value": "0", "module": "C3", "scenario": "S1"}, {"value": "0", "module": "C3", "scenario": "S2"}, {"value": "0", "module": "C4"}, {"value": "0", "module": "D", "scenario": "S1"}, {"value": "0", "module": "D", "scenario": "S2"}, {"value": "0", "module": "D", "scenario": "S3"}]}, "resolvedFlowVersion": "38.00.000", "flowProperties": [], "typeOfFlow": "Other flow", "classification": {"classHierarchy": "Quantities", "name": "GaBiCategories"}}, {"dataSetInternalID": 3, "referenceToFlowDataSet": {"shortDescription": [{"value": "Total erneuerbare Primärenergie (PERT)", "lang": "de"}, {"value": "Total use of renewable primary energy resources (PERT)", "lang": "en"}], "type": "flow data set", "refObjectId": "53f97275-fa8a-4cdd-9024-65936002acd0", "uri": "../flows/53f97275-fa8a-4cdd-9024-65936002acd0.xml"}, "exchange direction": "INPUT", "other": {"anies": [{"name": "referenceToUnitGroupDataSet", "value": {"shortDescription": [{"value": "MJ", "lang": "de"}], "type": "unit group data set", "refObjectId": "93a60a57-a3c8-11da-a746-0800200c9a66", "uri": "../unitgroups/93a60a57-a3c8-11da-a746-0800200c9a66.xml"}}, {"value": "69.3662340570049", "module": "A1-A3"}, {"value": "0.380564697823308", "module": "A4"}, {"value": "0.057320858356698", "module": "A5"}, {"value": "0", "module": "C1"}, {"value": "0.371853989685717", "module": "C2"}, {"value": "2.91095340873227", "module": "C3", "scenario": "S1"}, {"value": "47.1481094156143", "module": "C3", "scenario": "S2"}, {"value": "2.70343471790903", "module": "C4"}, {"value": "-4.62137284150507", "module": "D", "scenario": "S1"}, {"value": "-4.62137284150507", "module": "D", "scenario": "S2"}, {"value": "-4.62137284150507", "module": "D", "scenario": "S3"}]}, "resolvedFlowVersion": "38.00.000", "flowProperties": [], "typeOfFlow": "Other flow", "classification": {"classHierarchy": "Quantities / Environmental quantities / EPD EN 15804 / LCI indicators", "name": "GaBiCategories"}}, {"dataSetInternalID": 4, "referenceToFlowDataSet": {"shortDescription": [{"value": "Nicht-erneuerbare Primärenergie als Energieträger (PENRE)", "lang": "de"}, {"value": "Non renewable primary energy as energy carrier (PENRE)", "lang": "en"}], "type": "flow data set", "refObjectId": "ac857178-2b45-46ec-892a-a9a4332f0372", "uri": "../flows/ac857178-2b45-46ec-892a-a9a4332f0372.xml"}, "exchange direction": "INPUT", "other": {"anies": [{"name": "referenceToUnitGroupDataSet", "value": {"shortDescription": [{"value": "MJ", "lang": "de"}], "type": "unit group data set", "refObjectId": "93a60a57-a3c8-11da-a746-0800200c9a66", "uri": "../unitgroups/93a60a57-a3c8-11da-a746-0800200c9a66.xml"}}, {"value": "755.89911524491", "module": "A1-A3"}, {"value": "6.71034496308931", "module": "A4"}, {"value": "30.8791674468702", "module": "A5"}, {"value": "0", "module": "C1"}, {"value": "6.55675253370646", "module": "C2"}, {"value": "12.1569994986928", "module": "C3", "scenario": "S1"}, {"value": "84.9361415815311", "module": "C3", "scenario": "S2"}, {"value": "32.9003841652763", "module": "C4"}, {"value": "-16.7365525296792", "module": "D", "scenario": "S1"}, {"value": "-16.7365525296792", "module": "D", "scenario": "S2"}, {"value": "-16.7365525296792", "module": "D", "scenario": "S3"}]}, "resolvedFlowVersion": "38.00.000", "flowProperties": [], "typeOfFlow": "Other flow", "classification": {"classHierarchy": "Quantities", "name": "GaBiCategories"}}, {"dataSetInternalID": 5, "referenceToFlowDataSet": {"shortDescription": [{"value": "Nicht-erneuerbare Primärenergie zur stofflichen Nutzung (PENRM)", "lang": "de"}, {"value": "Non renewable primary energy as material utilization (PENRM)", "lang": "en"}], "type": "flow data set", "refObjectId": "1421caa0-679d-4bf4-b282-0eb850ccae27", "uri": "../flows/1421caa0-679d-4bf4-b282-0eb850ccae27.xml"}, "exchange direction": "INPUT", "other": {"anies": [{"name": "referenceToUnitGroupDataSet", "value": {"shortDescription": [{"value": "MJ", "lang": "de"}], "type": "unit group data set", "refObjectId": "93a60a57-a3c8-11da-a746-0800200c9a66", "uri": "../unitgroups/93a60a57-a3c8-11da-a746-0800200c9a66.xml"}}, {"value": "30.636", "module": "A1-A3"}, {"value": "0", "module": "A4"}, {"value": "-30.636", "module": "A5"}, {"value": "0", "module": "C1"}, {"value": "0", "module": "C2"}, {"value": "0", "module": "C3", "scenario": "S1"}, {"value": "0", "module": "C3", "scenario": "S2"}, {"value": "0", "module": "C4"}, {"value": "0", "module": "D", "scenario": "S1"}, {"value": "0", "module": "D", "scenario": "S2"}, {"value": "0", "module": "D", "scenario": "S3"}]}, "resolvedFlowVersion": "38.00.000", "flowProperties": [], "typeOfFlow": "Other flow", "classification": {"classHierarchy": "Quantities", "name": "GaBiCategories"}}, {"dataSetInternalID": 6, "referenceToFlowDataSet": {"shortDescription": [{"value": "Total nicht erneuerbare Primärenergie (PENRT)", "lang": "de"}, {"value": "Total use of non renewable primary energy resources (PENRT)", "lang": "en"}], "type": "flow data set", "refObjectId": "06159210-646b-4c8d-8583-da9b3b95a6c1", "uri": "../flows/06159210-646b-4c8d-8583-da9b3b95a6c1.xml"}, "exchange direction": "INPUT", "other": {"anies": [{"name": "referenceToUnitGroupDataSet", "value": {"shortDescription": [{"value": "MJ", "lang": "de"}], "type": "unit group data set", "refObjectId": "93a60a57-a3c8-11da-a746-0800200c9a66", "uri": "../unitgroups/93a60a57-a3c8-11da-a746-0800200c9a66.xml"}}, {"value": "786.535115244916", "module": "A1-A3"}, {"value": "6.71034496308931", "module": "A4"}, {"value": "0.243167446870181", "module": "A5"}, {"value": "0", "module": "C1"}, {"value": "6.55675253370646", "module": "C2"}, {"value": "12.1569994986928", "module": "C3", "scenario": "S1"}, {"value": "84.9361415815316", "module": "C3", "scenario": "S2"}, {"value": "32.9003841652766", "module": "C4"}, {"value": "-16.7365525296794", "module": "D", "scenario": "S1"}, {"value": "-16.7365525296793", "module": "D", "scenario": "S2"}, {"value": "-16.7365525296793", "module": "D", "scenario": "S3"}]}, "resolvedFlowVersion": "38.00.000", "flowProperties": [], "typeOfFlow": "Other flow", "classification": {"classHierarchy": "Quantities / Environmental quantities / EPD EN 15804 / LCI indicators", "name": "GaBiCategories"}}, {"dataSetInternalID": 7, "referenceToFlowDataSet": {"shortDescription": [{"value": "Einsatz von Sekundärstoffen (SM)", "lang": "de"}, {"value": "Use of secondary material (SM)", "lang": "en"}], "type": "flow data set", "refObjectId": "c6a1f35f-2d09-4f54-8dfb-97e502e1ce92", "uri": "../flows/c6a1f35f-2d09-4f54-8dfb-97e502e1ce92.xml"}, "exchange direction": "INPUT", "other": {"anies": [{"name": "referenceToUnitGroupDataSet", "value": {"shortDescription": [{"value": "kg", "lang": "de"}], "type": "unit group data set", "refObjectId": "ad38d542-3fe9-439d-9b95-2f5f7752acaf", "uri": "../unitgroups/ad38d542-3fe9-439d-9b95-2f5f7752acaf.xml"}}, {"value": "28.35", "module": "A1-A3"}, {"value": "0", "module": "A4"}, {"value": "0", "module": "A5"}, {"value": "0", "module": "C1"}, {"value": "0", "module": "C2"}, {"value": "0", "module": "C3", "scenario": "S1"}, {"value": "0", "module": "C3", "scenario": "S2"}, {"value": "0", "module": "C4"}, {"value": "0", "module": "D", "scenario": "S1"}, {"value": "0", "module": "D", "scenario": "S2"}, {"value": "0", "module": "D", "scenario": "S3"}]}, "resolvedFlowVersion": "38.00.000", "flowProperties": [], "typeOfFlow": "Other flow", "classification": {"classHierarchy": "Quantities / Environmental quantities / EPD EN 15804 / LCI indicators", "name": "GaBiCategories"}}, {"dataSetInternalID": 8, "referenceToFlowDataSet": {"shortDescription": [{"value": "Erneuerbare Sekundärbrennstoffe (RSF)", "lang": "de"}, {"value": "Use of renewable secondary fuels (RSF)", "lang": "en"}], "type": "flow data set", "refObjectId": "64333088-a55f-4aa2-9a31-c10b07816787", "uri": "../flows/64333088-a55f-4aa2-9a31-c10b07816787.xml"}, "exchange direction": "INPUT", "other": {"anies": [{"name": "referenceToUnitGroupDataSet", "value": {"shortDescription": [{"value": "MJ", "lang": "de"}], "type": "unit group data set", "refObjectId": "93a60a57-a3c8-11da-a746-0800200c9a66", "uri": "../unitgroups/93a60a57-a3c8-11da-a746-0800200c9a66.xml"}}, {"value": "0", "module": "A1-A3"}, {"value": "0", "module": "A4"}, {"value": "0", "module": "A5"}, {"value": "0", "module": "C1"}, {"value": "0", "module": "C2"}, {"value": "0", "module": "C3", "scenario": "S1"}, {"value": "0", "module": "C3", "scenario": "S2"}, {"value": "0", "module": "C4"}, {"value": "0", "module": "D", "scenario": "S1"}, {"value": "0", "module": "D", "scenario": "S2"}, {"value": "0", "module": "D", "scenario": "S3"}]}, "resolvedFlowVersion": "38.00.000", "flowProperties": [], "typeOfFlow": "Other flow", "classification": {"classHierarchy": "Quantities / Environmental quantities / EPD EN 15804 / LCI indicators", "name": "GaBiCategories"}}, {"dataSetInternalID": 9, "referenceToFlowDataSet": {"shortDescription": [{"value": "Nicht erneuerbare Sekundärbrennstoffe (NRSF)", "lang": "de"}, {"value": "Use of non renewable secondary fuels (NRSF)", "lang": "en"}], "type": "flow data set", "refObjectId": "89def144-d39a-4287-b86f-efde453ddcb2", "uri": "../flows/89def144-d39a-4287-b86f-efde453ddcb2.xml"}, "exchange direction": "INPUT", "other": {"anies": [{"name": "referenceToUnitGroupDataSet", "value": {"shortDescription": [{"value": "MJ", "lang": "de"}], "type": "unit group data set", "refObjectId": "93a60a57-a3c8-11da-a746-0800200c9a66", "uri": "../unitgroups/93a60a57-a3c8-11da-a746-0800200c9a66.xml"}}, {"value": "0", "module": "A1-A3"}, {"value": "0", "module": "A4"}, {"value": "0", "module": "A5"}, {"value": "0", "module": "C1"}, {"value": "0", "module": "C2"}, {"value": "0", "module": "C3", "scenario": "S1"}, {"value": "0", "module": "C3", "scenario": "S2"}, {"value": "0", "module": "C4"}, {"value": "0", "module": "D", "scenario": "S1"}, {"value": "0", "module": "D", "scenario": "S2"}, {"value": "0", "module": "D", "scenario": "S3"}]}, "resolvedFlowVersion": "38.00.000", "flowProperties": [], "typeOfFlow": "Other flow", "classification": {"classHierarchy": "Quantities / Environmental quantities / EPD EN 15804 / LCI indicators", "name": "GaBiCategories"}}, {"dataSetInternalID": 10, "referenceToFlowDataSet": {"shortDescription": [{"value": "Einsatz von Süßwasserressourcen (FW)", "lang": "de"}, {"value": "Use of net fresh water (FW)", "lang": "en"}], "type": "flow data set", "refObjectId": "3cf952c8-f3a4-461d-8c96-96456ca62246", "uri": "../flows/3cf952c8-f3a4-461d-8c96-96456ca62246.xml"}, "exchange direction": "INPUT", "other": {"anies": [{"name": "referenceToUnitGroupDataSet", "value": {"shortDescription": [{"value": "m^3", "lang": "de"}], "type": "unit group data set", "refObjectId": "cd950537-0a98-4044-9ba7-9f9a68d0a504", "uri": "../unitgroups/cd950537-0a98-4044-9ba7-9f9a68d0a504.xml"}}, {"value": "0.355480388419183", "module": "A1-A3"}, {"value": "0.000430399285559966", "module": "A4"}, {"value": "0.00450711180893672", "module": "A5"}, {"value": "0", "module": "C1"}, {"value": "0.000420547918419025", "module": "C2"}, {"value": "0.209528415286157", "module": "C3", "scenario": "S1"}, {"value": "0.0449764830923485", "module": "C3", "scenario": "S2"}, {"value": "0.000425681672110878", "module": "C4"}, {"value": "-0.0044422429815687", "module": "D", "scenario": "S1"}, {"value": "-0.00444224298156914", "module": "D", "scenario": "S2"}, {"value": "-0.00444224298156914", "module": "D", "scenario": "S3"}]}, "resolvedFlowVersion": "38.00.000", "flowProperties": [], "typeOfFlow": "Other flow", "classification": {"classHierarchy": "Quantities / Environmental quantities / EPD EN 15804 / LCI indicators", "name": "GaBiCategories"}}, {"dataSetInternalID": 11, "referenceToFlowDataSet": {"shortDescription": [{"value": "Gefährlicher Abfall zur Deponie (HWD)", "lang": "de"}, {"value": "Hazardous waste disposed (HWD)", "lang": "en"}], "type": "flow data set", "refObjectId": "430f9e0f-59b2-46a0-8e0d-55e0e84948fc", "uri": "../flows/430f9e0f-59b2-46a0-8e0d-55e0e84948fc.xml"}, "exchange direction": "OUTPUT", "other": {"anies": [{"name": "referenceToUnitGroupDataSet", "value": {"shortDescription": [{"value": "kg", "lang": "de"}], "type": "unit group data set", "refObjectId": "ad38d542-3fe9-439d-9b95-2f5f7752acaf", "uri": "../unitgroups/ad38d542-3fe9-439d-9b95-2f5f7752acaf.xml"}}, {"value": "5.98725392175687E-08", "module": "A1-A3"}, {"value": "3.21342290789893E-11", "module": "A4"}, {"value": "2.28784377311953E-11", "module": "A5"}, {"value": "0", "module": "C1"}, {"value": "3.13987118533123E-11", "module": "C2"}, {"value": "1.14081966128133E-09", "module": "C3", "scenario": "S1"}, {"value": "7.34972737829394E-09", "module": "C3", "scenario": "S2"}, {"value": "5.07256125031237E-09", "module": "C4"}, {"value": "-2.26146686990798E-09", "module": "D", "scenario": "S1"}, {"value": "-2.26146686990798E-09", "module": "D", "scenario": "S2"}, {"value": "-2.26146686990798E-09", "module": "D", "scenario": "S3"}]}, "resolvedFlowVersion": "38.00.000", "flowProperties": [], "typeOfFlow": "Other flow", "classification": {"classHierarchy": "Quantities / Environmental quantities / EPD EN 15804 / LCI indicators", "name": "GaBiCategories"}}, {"dataSetInternalID": 12, "referenceToFlowDataSet": {"shortDescription": [{"value": "Entsorgter nicht gefährlicher Abfall (NHWD)", "lang": "de"}, {"value": "Non hazardous waste disposed (NHWD)", "lang": "en"}], "type": "flow data set", "refObjectId": "b29ef66b-e286-4afa-949f-62f1a7b4d7fa", "uri": "../flows/b29ef66b-e286-4afa-949f-62f1a7b4d7fa.xml"}, "exchange direction": "OUTPUT", "other": {"anies": [{"name": "referenceToUnitGroupDataSet", "value": {"shortDescription": [{"value": "kg", "lang": "de"}], "type": "unit group data set", "refObjectId": "ad38d542-3fe9-439d-9b95-2f5f7752acaf", "uri": "../unitgroups/ad38d542-3fe9-439d-9b95-2f5f7752acaf.xml"}}, {"value": "1.30194017370916", "module": "A1-A3"}, {"value": "0.000961689268818195", "module": "A4"}, {"value": "0.0082679016492751", "module": "A5"}, {"value": "0", "module": "C1"}, {"value": "0.000939677257226886", "module": "C2"}, {"value": "0.62961627768512", "module": "C3", "scenario": "S1"}, {"value": "0.0639872711297903", "module": "C3", "scenario": "S2"}, {"value": "32.5698662927184", "module": "C4"}, {"value": "-0.00847795776796865", "module": "D", "scenario": "S1"}, {"value": "-0.00847795776796864", "module": "D", "scenario": "S2"}, {"value": "-0.00847795776796864", "module": "D", "scenario": "S3"}]}, "resolvedFlowVersion": "38.00.000", "flowProperties": [], "typeOfFlow": "Other flow", "classification": {"classHierarchy": "Quantities / Environmental quantities / EPD EN 15804 / LCI indicators", "name": "GaBiCategories"}}, {"dataSetInternalID": 13, "referenceToFlowDataSet": {"shortDescription": [{"value": "Entsorgter radioaktiver Abfall (RWD)", "lang": "de"}, {"value": "Radioactive waste disposed (RWD)", "lang": "en"}], "type": "flow data set", "refObjectId": "3449546e-52ad-4b39-b809-9fb77cea8ff6", "uri": "../flows/3449546e-52ad-4b39-b809-9fb77cea8ff6.xml"}, "exchange direction": "OUTPUT", "other": {"anies": [{"name": "referenceToUnitGroupDataSet", "value": {"shortDescription": [{"value": "kg", "lang": "de"}], "type": "unit group data set", "refObjectId": "ad38d542-3fe9-439d-9b95-2f5f7752acaf", "uri": "../unitgroups/ad38d542-3fe9-439d-9b95-2f5f7752acaf.xml"}}, {"value": "0.0413014827197804", "module": "A1-A3"}, {"value": "8.26496263653679E-06", "module": "A4"}, {"value": "1.47118835568625E-05", "module": "A5"}, {"value": "0", "module": "C1"}, {"value": "8.07578671531564E-06", "module": "C2"}, {"value": "0.000732742175905639", "module": "C3", "scenario": "S1"}, {"value": "0.0135763595250508", "module": "C3", "scenario": "S2"}, {"value": "0.000404064578844296", "module": "C4"}, {"value": "-0.00132525747422236", "module": "D", "scenario": "S1"}, {"value": "-0.00132525747422235", "module": "D", "scenario": "S2"}, {"value": "-0.00132525747422235", "module": "D", "scenario": "S3"}]}, "resolvedFlowVersion": "38.00.000", "flowProperties": [], "typeOfFlow": "Other flow", "classification": {"classHierarchy": "Quantities / Environmental quantities / EPD EN 15804 / LCI indicators", "name": "GaBiCategories"}}, {"dataSetInternalID": 14, "referenceToFlowDataSet": {"shortDescription": [{"value": "Komponenten für die Wiederverwendung (CRU)", "lang": "de"}, {"value": "Components for re-use (CRU)", "lang": "en"}], "type": "flow data set", "refObjectId": "a2b32f97-3fc7-4af2-b209-525bc6426f33", "uri": "../flows/a2b32f97-3fc7-4af2-b209-525bc6426f33.xml"}, "exchange direction": "OUTPUT", "other": {"anies": [{"name": "referenceToUnitGroupDataSet", "value": {"shortDescription": [{"value": "kg", "lang": "de"}], "type": "unit group data set", "refObjectId": "ad38d542-3fe9-439d-9b95-2f5f7752acaf", "uri": "../unitgroups/ad38d542-3fe9-439d-9b95-2f5f7752acaf.xml"}}, {"value": "0", "module": "A1-A3"}, {"value": "0", "module": "A4"}, {"value": "0", "module": "A5"}, {"value": "0", "module": "C1"}, {"value": "0", "module": "C2"}, {"value": "0", "module": "C3", "scenario": "S1"}, {"value": "0", "module": "C3", "scenario": "S2"}, {"value": "0", "module": "C4"}, {"value": "0", "module": "D", "scenario": "S1"}, {"value": "0", "module": "D", "scenario": "S2"}, {"value": "0", "module": "D", "scenario": "S3"}]}, "resolvedFlowVersion": "38.00.000", "flowProperties": [], "typeOfFlow": "Other flow", "classification": {"classHierarchy": "Quantities / Environmental quantities / EPD EN 15804 / LCI indicators", "name": "GaBiCategories"}}, {"dataSetInternalID": 15, "referenceToFlowDataSet": {"shortDescription": [{"value": "Stoffe zum Recycling (MFR)", "lang": "de"}, {"value": "Materials for recycling (MFR)", "lang": "en"}], "type": "flow data set", "refObjectId": "d7fe48a5-4103-49c8-9aae-b0b5dfdbd6ae", "uri": "../flows/d7fe48a5-4103-49c8-9aae-b0b5dfdbd6ae.xml"}, "exchange direction": "OUTPUT", "other": {"anies": [{"name": "referenceToUnitGroupDataSet", "value": {"shortDescription": [{"value": "kg", "lang": "de"}], "type": "unit group data set", "refObjectId": "ad38d542-3fe9-439d-9b95-2f5f7752acaf", "uri": "../unitgroups/ad38d542-3fe9-439d-9b95-2f5f7752acaf.xml"}}, {"value": "0", "module": "A1-A3"}, {"value": "0", "module": "A4"}, {"value": "0", "module": "A5"}, {"value": "0", "module": "C1"}, {"value": "0", "module": "C2"}, {"value": "0", "module": "C3", "scenario": "S1"}, {"value": "32.7", "module": "C3", "scenario": "S2"}, {"value": "0", "module": "C4"}, {"value": "0", "module": "D", "scenario": "S1"}, {"value": "0", "module": "D", "scenario": "S2"}, {"value": "0", "module": "D", "scenario": "S3"}]}, "resolvedFlowVersion": "38.00.000", "flowProperties": [], "typeOfFlow": "Other flow", "classification": {"classHierarchy": "Quantities / Environmental quantities / EPD EN 15804 / LCI indicators", "name": "GaBiCategories"}}, {"dataSetInternalID": 16, "referenceToFlowDataSet": {"shortDescription": [{"value": "Stoffe für die Energierückgewinnung (MER)", "lang": "de"}, {"value": "Materials for energy recovery (MER)", "lang": "en"}], "type": "flow data set", "refObjectId": "59a9181c-3aaf-46ee-8b13-2b3723b6e447", "uri": "../flows/59a9181c-3aaf-46ee-8b13-2b3723b6e447.xml"}, "exchange direction": "OUTPUT", "other": {"anies": [{"name": "referenceToUnitGroupDataSet", "value": {"shortDescription": [{"value": "kg", "lang": "de"}], "type": "unit group data set", "refObjectId": "ad38d542-3fe9-439d-9b95-2f5f7752acaf", "uri": "../unitgroups/ad38d542-3fe9-439d-9b95-2f5f7752acaf.xml"}}, {"value": "0", "module": "A1-A3"}, {"value": "0", "module": "A4"}, {"value": "0", "module": "A5"}, {"value": "0", "module": "C1"}, {"value": "0", "module": "C2"}, {"value": "0", "module": "C3", "scenario": "S1"}, {"value": "0", "module": "C3", "scenario": "S2"}, {"value": "0", "module": "C4"}, {"value": "0", "module": "D", "scenario": "S1"}, {"value": "0", "module": "D", "scenario": "S2"}, {"value": "0", "module": "D", "scenario": "S3"}]}, "resolvedFlowVersion": "38.00.000", "flowProperties": [], "typeOfFlow": "Other flow", "classification": {"classHierarchy": "Quantities / Environmental quantities / EPD EN 15804 / LCI indicators", "name": "GaBiCategories"}}, {"dataSetInternalID": 17, "referenceToFlowDataSet": {"shortDescription": [{"value": "Exportierte elektrische Energie (EEE)", "lang": "de"}, {"value": "Exported electrical energy (EEE)", "lang": "en"}], "type": "flow data set", "refObjectId": "4da0c987-2b76-40d6-9e9e-82a017aaaf29", "uri": "../flows/4da0c987-2b76-40d6-9e9e-82a017aaaf29.xml"}, "exchange direction": "OUTPUT", "other": {"anies": [{"name": "referenceToUnitGroupDataSet", "value": {"shortDescription": [{"value": "MJ", "lang": "de"}], "type": "unit group data set", "refObjectId": "93a60a57-a3c8-11da-a746-0800200c9a66", "uri": "../unitgroups/93a60a57-a3c8-11da-a746-0800200c9a66.xml"}}, {"value": "0", "module": "A1-A3"}, {"value": "0", "module": "A4"}, {"value": "4.44963923895632", "module": "A5"}, {"value": "0", "module": "C1"}, {"value": "0", "module": "C2"}, {"value": "198.268363906412", "module": "C3", "scenario": "S1"}, {"value": "0", "module": "C3", "scenario": "S2"}, {"value": "0", "module": "C4"}, {"value": "0", "module": "D", "scenario": "S1"}, {"value": "0", "module": "D", "scenario": "S2"}, {"value": "0", "module": "D", "scenario": "S3"}]}, "resolvedFlowVersion": "38.00.000", "flowProperties": [], "typeOfFlow": "Other flow", "classification": {"classHierarchy": "Quantities / Environmental quantities / EPD EN 15804 / LCI indicators", "name": "GaBiCategories"}}, {"dataSetInternalID": 18, "referenceToFlowDataSet": {"shortDescription": [{"value": "Exportierte thermische Energie (EET)", "lang": "de"}, {"value": "Exported thermal energy (EET)", "lang": "en"}], "type": "flow data set", "refObjectId": "98daf38a-7a79-46d3-9a37-2b7bd0955810", "uri": "../flows/98daf38a-7a79-46d3-9a37-2b7bd0955810.xml"}, "exchange direction": "OUTPUT", "other": {"anies": [{"name": "referenceToUnitGroupDataSet", "value": {"shortDescription": [{"value": "MJ", "lang": "de"}], "type": "unit group data set", "refObjectId": "93a60a57-a3c8-11da-a746-0800200c9a66", "uri": "../unitgroups/93a60a57-a3c8-11da-a746-0800200c9a66.xml"}}, {"value": "0", "module": "A1-A3"}, {"value": "0", "module": "A4"}, {"value": "7.91206989181843", "module": "A5"}, {"value": "0", "module": "C1"}, {"value": "0", "module": "C2"}, {"value": "353.380732856254", "module": "C3", "scenario": "S1"}, {"value": "0", "module": "C3", "scenario": "S2"}, {"value": "0", "module": "C4"}, {"value": "0", "module": "D", "scenario": "S1"}, {"value": "0", "module": "D", "scenario": "S2"}, {"value": "0", "module": "D", "scenario": "S3"}]}, "resolvedFlowVersion": "38.00.000", "flowProperties": [], "typeOfFlow": "Other flow", "classification": {"classHierarchy": "Quantities / Environmental quantities / EPD EN 15804 / LCI indicators", "name": "GaBiCategories"}}]}, "LCIAResults": {"LCIAResult": [{"referenceToLCIAMethodDataSet": {"shortDescription": [{"value": "Globales Erwärmungspotenzial total (GWP-total)", "lang": "de"}, {"value": "Global Warming Potential total (GWP-total)", "lang": "en"}], "type": "LCIA method data set", "refObjectId": "6a37f984-a4b3-458a-a20a-64418c145fa2", "uri": "../lciamethods/6a37f984-a4b3-458a-a20a-64418c145fa2.xml"}, "other": {"anies": [{"name": "referenceToUnitGroupDataSet", "value": {"shortDescription": [{"value": "kg CO_(2)-Äq.", "lang": "de"}], "type": "unit group data set", "refObjectId": "1ebf3012-d0db-4de2-aefd-ef30cedb0be1", "uri": "../unitgroups/1ebf3012-d0db-4de2-aefd-ef30cedb0be1.xml"}}, {"value": "54.2416173425411", "module": "A1-A3"}, {"value": "0.505978533743402", "module": "A4"}, {"value": "2.08579186454395", "module": "A5"}, {"value": "0", "module": "C1"}, {"value": "0.49439724058475", "module": "C2"}, {"value": "109.524872552716", "module": "C3", "scenario": "S1"}, {"value": "4.72339255275829", "module": "C3", "scenario": "S2"}, {"value": "2.29404350354312", "module": "C4"}, {"value": "-0.988747743213216", "module": "D", "scenario": "S1"}, {"value": "-0.988747743213215", "module": "D", "scenario": "S2"}, {"value": "-0.988747743213215", "module": "D", "scenario": "S3"}]}}, {"referenceToLCIAMethodDataSet": {"shortDescription": [{"value": "Globales Erwärmungspotenzial fossil (GWP-fossil)", "lang": "de"}, {"value": "Global Warming Potential fossil fuels (GWP-fossil)", "lang": "en"}], "type": "LCIA method data set", "refObjectId": "5f635281-343e-44fb-83df-1971b155e6b6", "uri": "../lciamethods/5f635281-343e-44fb-83df-1971b155e6b6.xml"}, "other": {"anies": [{"name": "referenceToUnitGroupDataSet", "value": {"shortDescription": [{"value": "kg CO_(2)-Äq.", "lang": "de"}], "type": "unit group data set", "refObjectId": "1ebf3012-d0db-4de2-aefd-ef30cedb0be1", "uri": "../unitgroups/1ebf3012-d0db-4de2-aefd-ef30cedb0be1.xml"}}, {"value": "53.5854457538056", "module": "A1-A3"}, {"value": "0.503032438067318", "module": "A4"}, {"value": "2.08572267256713", "module": "A5"}, {"value": "0", "module": "C1"}, {"value": "0.491518577804377", "module": "C2"}, {"value": "109.521475825962", "module": "C3", "scenario": "S1"}, {"value": "4.68025319491255", "module": "C3", "scenario": "S2"}, {"value": "2.31758120291474", "module": "C4"}, {"value": "-0.983588205848648", "module": "D", "scenario": "S1"}, {"value": "-0.983588205848647", "module": "D", "scenario": "S2"}, {"value": "-0.983588205848647", "module": "D", "scenario": "S3"}]}}, {"referenceToLCIAMethodDataSet": {"shortDescription": [{"value": "Globales Erwärmungspotenzial biogen (GWP-biogenic)", "lang": "de"}, {"value": "Global Warming Potential biogenic (GWP-biogenic)", "lang": "en"}], "type": "LCIA method data set", "refObjectId": "2356e1ab-0185-4db5-86e5-16de51c7485c", "uri": "../lciamethods/2356e1ab-0185-4db5-86e5-16de51c7485c.xml"}, "other": {"anies": [{"name": "referenceToUnitGroupDataSet", "value": {"shortDescription": [{"value": "kg CO_(2)-Äq.", "lang": "de"}], "type": "unit group data set", "refObjectId": "1ebf3012-d0db-4de2-aefd-ef30cedb0be1", "uri": "../unitgroups/1ebf3012-d0db-4de2-aefd-ef30cedb0be1.xml"}}, {"value": "0.629729117633922", "module": "A1-A3"}, {"value": "0.000153239917592734", "module": "A4"}, {"value": "6.69918372814759E-05", "module": "A5"}, {"value": "0", "module": "C1"}, {"value": "0.00014973242411051", "module": "C2"}, {"value": "0.00326822816088908", "module": "C3", "scenario": "S1"}, {"value": "0.042149522765073", "module": "C3", "scenario": "S2"}, {"value": "-0.0246659866726582", "module": "C4"}, {"value": "-0.0050509123910121", "module": "D", "scenario": "S1"}, {"value": "-0.00505091239101209", "module": "D", "scenario": "S2"}, {"value": "-0.00505091239101209", "module": "D", "scenario": "S3"}]}}, {"referenceToLCIAMethodDataSet": {"shortDescription": [{"value": "Globales Erwärmungspotenzial luluc (GWP-luluc)", "lang": "de"}, {"value": "Global Warming Potential luluc (GWP-luluc)", "lang": "en"}], "type": "LCIA method data set", "refObjectId": "4331bbdb-978a-490d-8707-eeb047f01a55", "uri": "../lciamethods/4331bbdb-978a-490d-8707-eeb047f01a55.xml"}, "other": {"anies": [{"name": "referenceToUnitGroupDataSet", "value": {"shortDescription": [{"value": "kg CO_(2)-Äq.", "lang": "de"}], "type": "unit group data set", "refObjectId": "1ebf3012-d0db-4de2-aefd-ef30cedb0be1", "uri": "../unitgroups/1ebf3012-d0db-4de2-aefd-ef30cedb0be1.xml"}}, {"value": "0.0264424711016876", "module": "A1-A3"}, {"value": "0.00279285575849096", "module": "A4"}, {"value": "2.20013954173603E-06", "module": "A5"}, {"value": "0", "module": "C1"}, {"value": "0.00272893035626171", "module": "C2"}, {"value": "0.000128498592863911", "module": "C3", "scenario": "S1"}, {"value": "0.000989835080670853", "module": "C3", "scenario": "S2"}, {"value": "0.00112828730103577", "module": "C4"}, {"value": "-0.000108624973556288", "module": "D", "scenario": "S1"}, {"value": "-0.000108624973556288", "module": "D", "scenario": "S2"}, {"value": "-0.000108624973556288", "module": "D", "scenario": "S3"}]}}, {"referenceToLCIAMethodDataSet": {"shortDescription": [{"value": "Abbau Potential der stratosphärischen Ozonschicht (ODP)", "lang": "de"}, {"value": "Depletion potential of the stratospheric ozone layer (ODP)", "lang": "en"}], "type": "LCIA method data set", "refObjectId": "b5c629d6-def3-11e6-bf01-fe55135034f3", "uri": "../lciamethods/b5c629d6-def3-11e6-bf01-fe55135034f3.xml"}, "other": {"anies": [{"name": "referenceToUnitGroupDataSet", "value": {"shortDescription": [{"value": "kg CFC11-Äq.", "lang": "de"}], "type": "unit group data set", "refObjectId": "d9e957c9-7309-4474-bf3a-7777df6c4e5b", "uri": "../unitgroups/d9e957c9-7309-4474-bf3a-7777df6c4e5b.xml"}}, {"value": "1.72094672599029E-10", "module": "A1-A3"}, {"value": "3.00122045315758E-14", "module": "A4"}, {"value": "8.93645019331017E-14", "module": "A5"}, {"value": "0", "module": "C1"}, {"value": "2.93252581181656E-14", "module": "C2"}, {"value": "4.58404766845644E-12", "module": "C3", "scenario": "S1"}, {"value": "6.85138485625513E-11", "module": "C3", "scenario": "S2"}, {"value": "3.11297071052921E-12", "module": "C4"}, {"value": "-6.68984792381944E-12", "module": "D", "scenario": "S1"}, {"value": "-6.68984792381943E-12", "module": "D", "scenario": "S2"}, {"value": "-6.68984792381943E-12", "module": "D", "scenario": "S3"}]}}, {"referenceToLCIAMethodDataSet": {"shortDescription": [{"value": "Versauerungspotenzial von Boden und Wasser (AP)", "lang": "de"}, {"value": "Acidification potential of land and water (AP)", "lang": "en"}], "type": "LCIA method data set", "refObjectId": "b5c611c6-def3-11e6-bf01-fe55135034f3", "uri": "../lciamethods/b5c611c6-def3-11e6-bf01-fe55135034f3.xml"}, "other": {"anies": [{"name": "referenceToUnitGroupDataSet", "value": {"shortDescription": [{"value": "mol H^(+)-Äq.", "lang": "de"}], "type": "unit group data set", "refObjectId": "42e089ac-92bf-4bf2-8ca1-5fc40d18f2ed", "uri": "../unitgroups/42e089ac-92bf-4bf2-8ca1-5fc40d18f2ed.xml"}}, {"value": "0.0927437886777657", "module": "A1-A3"}, {"value": "0.000476746532501729", "module": "A4"}, {"value": "0.000207085444891648", "module": "A5"}, {"value": "0", "module": "C1"}, {"value": "0.000465834327759712", "module": "C2"}, {"value": "0.0096355764842797", "module": "C3", "scenario": "S1"}, {"value": "0.0102732295469091", "module": "C3", "scenario": "S2"}, {"value": "0.0068687339713351", "module": "C4"}, {"value": "-0.00129824270638087", "module": "D", "scenario": "S1"}, {"value": "-0.00129824270638087", "module": "D", "scenario": "S2"}, {"value": "-0.00129824270638087", "module": "D", "scenario": "S3"}]}}, {"referenceToLCIAMethodDataSet": {"shortDescription": [{"value": "Eutrophierungspotenzial Süßwasser (EP-freshwater)", "lang": "de"}, {"value": "Eutrophication potential aquatic freshwater (EP-freshwater)", "lang": "en"}], "type": "LCIA method data set", "refObjectId": "b53ec18f-7377-4ad3-86eb-cc3f4f276b2b", "uri": "../lciamethods/b53ec18f-7377-4ad3-86eb-cc3f4f276b2b.xml"}, "other": {"anies": [{"name": "referenceToUnitGroupDataSet", "value": {"shortDescription": [{"value": "kg P-Äq.", "lang": "de"}], "type": "unit group data set", "refObjectId": "0429039d-a61d-4590-ba67-aa4a20a810a1", "uri": "../unitgroups/0429039d-a61d-4590-ba67-aa4a20a810a1.xml"}}, {"value": "0.000104659984877688", "module": "A1-A3"}, {"value": "1.49527924902206E-06", "module": "A4"}, {"value": "2.08324109659875E-08", "module": "A5"}, {"value": "0", "module": "C1"}, {"value": "1.46105394857531E-06", "module": "C2"}, {"value": "1.07260207972614E-06", "module": "C3", "scenario": "S1"}, {"value": "1.36549221296706E-05", "module": "C3", "scenario": "S2"}, {"value": "0.000432625099038477", "module": "C4"}, {"value": "-1.36090593669381E-06", "module": "D", "scenario": "S1"}, {"value": "-1.36090593669381E-06", "module": "D", "scenario": "S2"}, {"value": "-1.36090593669381E-06", "module": "D", "scenario": "S3"}]}}, {"referenceToLCIAMethodDataSet": {"shortDescription": [{"value": "Eutrophierungspotenzial Salzwasser (EP-marine)", "lang": "de"}, {"value": "Eutrophication potential aquatic marine (EP-marine)", "lang": "en"}], "type": "LCIA method data set", "refObjectId": "b5c619fa-def3-11e6-bf01-fe55135034f3", "uri": "../lciamethods/b5c619fa-def3-11e6-bf01-fe55135034f3.xml"}, "other": {"anies": [{"name": "referenceToUnitGroupDataSet", "value": {"shortDescription": [{"value": "kg N-Äq.", "lang": "de"}], "type": "unit group data set", "refObjectId": "d05bb823-ecdf-4686-8c40-bf1d9257859f", "uri": "../unitgroups/d05bb823-ecdf-4686-8c40-bf1d9257859f.xml"}}, {"value": "0.0337445670364842", "module": "A1-A3"}, {"value": "0.000148533528048423", "module": "A4"}, {"value": "4.31844722110535E-05", "module": "A5"}, {"value": "0", "module": "C1"}, {"value": "0.000145133758656052", "module": "C2"}, {"value": "0.00211291821652235", "module": "C3", "scenario": "S1"}, {"value": "0.00230524216807324", "module": "C3", "scenario": "S2"}, {"value": "0.00151961721704246", "module": "C4"}, {"value": "-0.000351694161555714", "module": "D", "scenario": "S1"}, {"value": "-0.000351694161555713", "module": "D", "scenario": "S2"}, {"value": "-0.000351694161555713", "module": "D", "scenario": "S3"}]}}, {"referenceToLCIAMethodDataSet": {"shortDescription": [{"value": "Eutrophierungspotenzial Land (EP-terrestrial)", "lang": "de"}, {"value": "Eutrophication potential terrestrial (EP-terrestrial)", "lang": "en"}], "type": "LCIA method data set", "refObjectId": "b5c614d2-def3-11e6-bf01-fe55135034f3", "uri": "../lciamethods/b5c614d2-def3-11e6-bf01-fe55135034f3.xml"}, "other": {"anies": [{"name": "referenceToUnitGroupDataSet", "value": {"shortDescription": [{"value": "mol N-Äq.", "lang": "de"}], "type": "unit group data set", "refObjectId": "71b4d617-0ec9-4d3f-b65e-e438940c2401", "uri": "../unitgroups/71b4d617-0ec9-4d3f-b65e-e438940c2401.xml"}}, {"value": "0.376345213504446", "module": "A1-A3"}, {"value": "0.00178421151232737", "module": "A4"}, {"value": "0.000970123654225734", "module": "A5"}, {"value": "0", "module": "C1"}, {"value": "0.00174337286957225", "module": "C2"}, {"value": "0.0452107128041993", "module": "C3", "scenario": "S1"}, {"value": "0.0241845609219681", "module": "C3", "scenario": "S2"}, {"value": "0.0166665636151257", "module": "C4"}, {"value": "-0.00376610774166575", "module": "D", "scenario": "S1"}, {"value": "-0.00376610774166575", "module": "D", "scenario": "S2"}, {"value": "-0.00376610774166575", "module": "D", "scenario": "S3"}]}}, {"referenceToLCIAMethodDataSet": {"shortDescription": [{"value": "Bildungspotential für troposphärisches Ozon (POCP)", "lang": "de"}, {"value": "Formation potential of tropospheric ozone photochemical oxidants (POCP)", "lang": "en"}], "type": "LCIA method data set", "refObjectId": "b5c610fe-def3-11e6-bf01-fe55135034f3", "uri": "../lciamethods/b5c610fe-def3-11e6-bf01-fe55135034f3.xml"}, "other": {"anies": [{"name": "referenceToUnitGroupDataSet", "value": {"shortDescription": [{"value": "kg NMVOC-Äq.", "lang": "de"}], "type": "unit group data set", "refObjectId": "d27c25f8-fbc1-44c6-b47b-4adbae4199c6", "uri": "../unitgroups/d27c25f8-fbc1-44c6-b47b-4adbae4199c6.xml"}}, {"value": "0.444705202137617", "module": "A1-A3"}, {"value": "0.000415403129350068", "module": "A4"}, {"value": "0.000128583026345976", "module": "A5"}, {"value": "0", "module": "C1"}, {"value": "0.000405895007761526", "module": "C2"}, {"value": "0.00622607350354244", "module": "C3", "scenario": "S1"}, {"value": "0.00623100308024436", "module": "C3", "scenario": "S2"}, {"value": "0.00488857384328252", "module": "C4"}, {"value": "-0.000984054926215206", "module": "D", "scenario": "S1"}, {"value": "-0.000984054926215205", "module": "D", "scenario": "S2"}, {"value": "-0.000984054926215205", "module": "D", "scenario": "S3"}]}}, {"referenceToLCIAMethodDataSet": {"shortDescription": [{"value": "Potenzial für den abiotischen Abbau nicht fossiler Ressourcen (ADPE)", "lang": "de"}, {"value": "Abiotic depletion potential for non fossil resources (ADPE)", "lang": "en"}], "type": "LCIA method data set", "refObjectId": "b2ad6494-c78d-11e6-9d9d-cec0c932ce01", "uri": "../lciamethods/b2ad6494-c78d-11e6-9d9d-cec0c932ce01.xml"}, "other": {"anies": [{"name": "referenceToUnitGroupDataSet", "value": {"shortDescription": [{"value": "kg Sb-Äq.", "lang": "de"}], "type": "unit group data set", "refObjectId": "54ccd2d9-a32a-4fc2-923d-f2c8c93e89d4", "uri": "../unitgroups/54ccd2d9-a32a-4fc2-923d-f2c8c93e89d4.xml"}}, {"value": "4.93357339001592E-06", "module": "A1-A3"}, {"value": "4.18770523860859E-08", "module": "A4"}, {"value": "2.16357986370536E-09", "module": "A5"}, {"value": "0", "module": "C1"}, {"value": "4.09185326308793E-08", "module": "C2"}, {"value": "1.10893716712797E-07", "module": "C3", "scenario": "S1"}, {"value": "1.27530535035231E-06", "module": "C3", "scenario": "S2"}, {"value": "1.60721831847868E-07", "module": "C4"}, {"value": "-1.49022936339299E-07", "module": "D", "scenario": "S1"}, {"value": "-1.49022936339299E-07", "module": "D", "scenario": "S2"}, {"value": "-1.49022936339299E-07", "module": "D", "scenario": "S3"}]}}, {"referenceToLCIAMethodDataSet": {"shortDescription": [{"value": "Potenzial für den abiotischen Abbau fossiler Brennstoffe (ADPF)", "lang": "de"}, {"value": "Abiotic depletion potential for fossil resources (ADPF)", "lang": "en"}], "type": "LCIA method data set", "refObjectId": "b2ad6110-c78d-11e6-9d9d-cec0c932ce01", "uri": "../lciamethods/b2ad6110-c78d-11e6-9d9d-cec0c932ce01.xml"}, "other": {"anies": [{"name": "referenceToUnitGroupDataSet", "value": {"shortDescription": [{"value": "MJ", "lang": "de"}], "type": "unit group data set", "refObjectId": "93a60a57-a3c8-11da-a746-0800200c9a66", "uri": "../unitgroups/93a60a57-a3c8-11da-a746-0800200c9a66.xml"}}, {"value": "786.042540161719", "module": "A1-A3"}, {"value": "6.69433425134597", "module": "A4"}, {"value": "0.242971655754008", "module": "A5"}, {"value": "0", "module": "C1"}, {"value": "6.54110828957788", "module": "C2"}, {"value": "12.147261975817", "module": "C3", "scenario": "S1"}, {"value": "84.9144334009367", "module": "C3", "scenario": "S2"}, {"value": "32.8876766858904", "module": "C4"}, {"value": "-16.7342893435999", "module": "D", "scenario": "S1"}, {"value": "-16.7342893435999", "module": "D", "scenario": "S2"}, {"value": "-16.7342893435999", "module": "D", "scenario": "S3"}]}}, {"referenceToLCIAMethodDataSet": {"shortDescription": [{"value": "Wassernutzung (WDP)", "lang": "de"}, {"value": "Water use (WDP)", "lang": "en"}], "type": "LCIA method data set", "refObjectId": "b2ad66ce-c78d-11e6-9d9d-cec0c932ce01", "uri": "../lciamethods/b2ad66ce-c78d-11e6-9d9d-cec0c932ce01.xml"}, "other": {"anies": [{"name": "referenceToUnitGroupDataSet", "value": {"shortDescription": [{"value": "m^(3) Welt-Äq. entzogen", "lang": "de"}], "type": "unit group data set", "refObjectId": "6ae2df01-888e-46c8-b17d-49fa3869b476", "uri": "../unitgroups/6ae2df01-888e-46c8-b17d-49fa3869b476.xml"}}, {"value": "1.89094522266641", "module": "A1-A3"}, {"value": "0.004493350780088", "module": "A4"}, {"value": "0.192425191757818", "module": "A5"}, {"value": "0", "module": "C1"}, {"value": "0.00439050291366977", "module": "C2"}, {"value": "8.9410198989095", "module": "C3", "scenario": "S1"}, {"value": "1.06747498754061", "module": "C3", "scenario": "S2"}, {"value": "-0.022848841151351", "module": "C4"}, {"value": "-0.105380123213092", "module": "D", "scenario": "S1"}, {"value": "-0.105380123213077", "module": "D", "scenario": "S2"}, {"value": "-0.105380123213077", "module": "D", "scenario": "S3"}]}}, {"referenceToLCIAMethodDataSet": {"shortDescription": [{"value": "Auftreten von Krankheiten aufgrund von Feinstaubemissionen (PM)", "lang": "de"}, {"value": "Incidence of disease due to PM emissions (PM)", "lang": "en"}], "type": "LCIA method data set", "refObjectId": "b5c602c6-def3-11e6-bf01-fe55135034f3", "uri": "../lciamethods/b5c602c6-def3-11e6-bf01-fe55135034f3.xml"}, "other": {"anies": [{"name": "referenceToUnitGroupDataSet", "value": {"shortDescription": [{"value": "Krankheitsfälle", "lang": "de"}], "type": "unit group data set", "refObjectId": "3883559b-648f-4afc-8ba2-0bd24f3affa3", "uri": "../unitgroups/3883559b-648f-4afc-8ba2-0bd24f3affa3.xml"}}, {"value": "1.54849377676373E-06", "module": "A1-A3"}, {"value": "2.88386550570226E-09", "module": "A4"}, {"value": "1.20985987518605E-09", "module": "A5"}, {"value": "0", "module": "C1"}, {"value": "2.81785699027263E-09", "module": "C2"}, {"value": "5.60914938314854E-08", "module": "C3", "scenario": "S1"}, {"value": "8.51692999753763E-08", "module": "C3", "scenario": "S2"}, {"value": "6.6012098975617E-08", "module": "C4"}, {"value": "-1.07538199793373E-08", "module": "D", "scenario": "S1"}, {"value": "-1.07538199793373E-08", "module": "D", "scenario": "S2"}, {"value": "-1.07538199793373E-08", "module": "D", "scenario": "S3"}]}}, {"referenceToLCIAMethodDataSet": {"shortDescription": [{"value": "Wirkung durch Exposition des Menschen mit U235 (IR)", "lang": "de"}, {"value": "Human exposure efficiency relative to U235 (IR)", "lang": "en"}], "type": "LCIA method data set", "refObjectId": "b5c632be-def3-11e6-bf01-fe55135034f3", "uri": "../lciamethods/b5c632be-def3-11e6-bf01-fe55135034f3.xml"}, "other": {"anies": [{"name": "referenceToUnitGroupDataSet", "value": {"shortDescription": [{"value": "kBq U235-Äq.", "lang": "de"}], "type": "unit group data set", "refObjectId": "456b05bf-1415-44a9-9993-02452f554c09", "uri": "../unitgroups/456b05bf-1415-44a9-9993-02452f554c09.xml"}}, {"value": "3.44011676292795", "module": "A1-A3"}, {"value": "0.00121115560200501", "module": "A4"}, {"value": "0.00241460555521408", "module": "A5"}, {"value": "0", "module": "C1"}, {"value": "0.00118343357991883", "module": "C2"}, {"value": "0.119613270078725", "module": "C3", "scenario": "S1"}, {"value": "2.29993091971019", "module": "C3", "scenario": "S2"}, {"value": "0.0596467181399746", "module": "C4"}, {"value": "-0.224399121546436", "module": "D", "scenario": "S1"}, {"value": "-0.224399121546436", "module": "D", "scenario": "S2"}, {"value": "-0.224399121546436", "module": "D", "scenario": "S3"}]}}, {"referenceToLCIAMethodDataSet": {"shortDescription": [{"value": "Toxizitätsvergleichseinheit für Ökosysteme (ETP-fw)", "lang": "de"}, {"value": "Comparative toxic unit for ecosystems (ETP-fw)", "lang": "en"}], "type": "LCIA method data set", "refObjectId": "ee1082d1-b0f7-43ca-a1f0-21e2a4a74511", "uri": "../lciamethods/ee1082d1-b0f7-43ca-a1f0-21e2a4a74511.xml"}, "other": {"anies": [{"name": "referenceToUnitGroupDataSet", "value": {"shortDescription": [{"value": "CTUe", "lang": "de"}], "type": "unit group data set", "refObjectId": "aa959ded-f1eb-4efb-9c5c-2d60be36b3e6", "uri": "../unitgroups/aa959ded-f1eb-4efb-9c5c-2d60be36b3e6.xml"}}, {"value": "401.356514919374", "module": "A1-A3"}, {"value": "4.64752484867131", "module": "A4"}, {"value": "0.112479886858399", "module": "A5"}, {"value": "0", "module": "C1"}, {"value": "4.54114810708038", "module": "C2"}, {"value": "5.95908519148633", "module": "C3", "scenario": "S1"}, {"value": "37.1988739732473", "module": "C3", "scenario": "S2"}, {"value": "32.1836704982373", "module": "C4"}, {"value": "-3.693838175231", "module": "D", "scenario": "S1"}, {"value": "-3.69383817523099", "module": "D", "scenario": "S2"}, {"value": "-3.69383817523099", "module": "D", "scenario": "S3"}]}}, {"referenceToLCIAMethodDataSet": {"shortDescription": [{"value": "Toxizitätsvergleichseinheit für Menschen (krebserregend) (HTP-c)", "lang": "de"}, {"value": "Comparative toxic unit for humans (carcinogenic) (HTP-c)", "lang": "en"}], "type": "LCIA method data set", "refObjectId": "2299222a-bbd8-474f-9d4f-4dd1f18aea7c", "uri": "../lciamethods/2299222a-bbd8-474f-9d4f-4dd1f18aea7c.xml"}, "other": {"anies": [{"name": "referenceToUnitGroupDataSet", "value": {"shortDescription": [{"value": "CTUh", "lang": "de"}], "type": "unit group data set", "refObjectId": "d4c9523e-2d7e-49fd-8469-998f547d3a70", "uri": "../unitgroups/d4c9523e-2d7e-49fd-8469-998f547d3a70.xml"}}, {"value": "7.19652137284507E-09", "module": "A1-A3"}, {"value": "9.36716453654082E-11", "module": "A4"}, {"value": "1.3280038196257E-11", "module": "A5"}, {"value": "0", "module": "C1"}, {"value": "9.15276042385958E-11", "module": "C2"}, {"value": "6.00468105636009E-10", "module": "C3", "scenario": "S1"}, {"value": "1.06842557832315E-09", "module": "C3", "scenario": "S2"}, {"value": "1.44511680930355E-09", "module": "C4"}, {"value": "-1.69023742636932E-10", "module": "D", "scenario": "S1"}, {"value": "-1.69023742636932E-10", "module": "D", "scenario": "S2"}, {"value": "-1.69023742636932E-10", "module": "D", "scenario": "S3"}]}}, {"referenceToLCIAMethodDataSet": {"shortDescription": [{"value": "Toxizitätsvergleichseinheit für Menschen (nicht krebserregend) (HTP-nc)", "lang": "de"}, {"value": "Comparative toxic unit for humans (noncarcinogenic) (HTP-nc)", "lang": "en"}], "type": "LCIA method data set", "refObjectId": "3af763a5-b7a1-48c9-9cee-1f223481fcef", "uri": "../lciamethods/3af763a5-b7a1-48c9-9cee-1f223481fcef.xml"}, "other": {"anies": [{"name": "referenceToUnitGroupDataSet", "value": {"shortDescription": [{"value": "CTUh", "lang": "de"}], "type": "unit group data set", "refObjectId": "d4c9523e-2d7e-49fd-8469-998f547d3a70", "uri": "../unitgroups/d4c9523e-2d7e-49fd-8469-998f547d3a70.xml"}}, {"value": "3.97117277669555E-07", "module": "A1-A3"}, {"value": "4.84627595599324E-09", "module": "A4"}, {"value": "4.13542633638691E-10", "module": "A5"}, {"value": "0", "module": "C1"}, {"value": "4.73535001975076E-09", "module": "C2"}, {"value": "1.95164742495441E-08", "module": "C3", "scenario": "S1"}, {"value": "3.90773126676623E-08", "module": "C3", "scenario": "S2"}, {"value": "1.21118293582757E-07", "module": "C4"}, {"value": "-6.48939586968594E-09", "module": "D", "scenario": "S1"}, {"value": "-6.48939586968593E-09", "module": "D", "scenario": "S2"}, {"value": "-6.48939586968593E-09", "module": "D", "scenario": "S3"}]}}, {"referenceToLCIAMethodDataSet": {"shortDescription": [{"value": "Bodenqualitätsindex (SQP)", "lang": "de"}, {"value": "Soil quality index (SQP)", "lang": "en"}], "type": "LCIA method data set", "refObjectId": "b2ad6890-c78d-11e6-9d9d-cec0c932ce01", "uri": "../lciamethods/b2ad6890-c78d-11e6-9d9d-cec0c932ce01.xml"}, "other": {"anies": [{"name": "referenceToUnitGroupDataSet", "value": {"shortDescription": [{"value": "SQP", "lang": "de"}], "type": "unit group data set", "refObjectId": "f130951c-e67f-4f7f-8dd4-665de3974e18", "uri": "../unitgroups/f130951c-e67f-4f7f-8dd4-665de3974e18.xml"}}, {"value": "60.0734712503925", "module": "A1-A3"}, {"value": "2.30350957042895", "module": "A4"}, {"value": "0.0735267129484151", "module": "A5"}, {"value": "0", "module": "C1"}, {"value": "2.2507847652252", "module": "C2"}, {"value": "3.69087283810418", "module": "C3", "scenario": "S1"}, {"value": "30.6220488587394", "module": "C3", "scenario": "S2"}, {"value": "2.36626172624778", "module": "C4"}, {"value": "-3.00132421930618", "module": "D", "scenario": "S1"}, {"value": "-3.00132421930618", "module": "D", "scenario": "S2"}, {"value": "-3.00132421930618", "module": "D", "scenario": "S3"}]}}]}, "otherAttributes": {"{http://www.indata.network/EPD/2019}epd-version": "1.2"}, "version": "1.1", "locations": "../ILCDLocations.xml"}