{"processInformation": {"dataSetInformation": {"UUID": "650a4800-0bc1-4d1e-b673-85e05cfc2310", "name": {"baseName": [{"value": "Außenliegender Raffstore", "lang": "de"}, {"value": "External Venetian Blind", "lang": "en"}], "functionalUnitFlowProperties": [{"lang": "de"}]}, "classificationInformation": {"classification": [{"class": [{"value": "Komponenten von Fenstern und Vorhangfassaden", "level": 0, "classId": "7"}, {"value": "Zubehör für Fenster, Fassaden, Türen und Tore", "level": 1, "classId": "7.11"}, {"value": "Sonnenschutzsysteme", "level": 2, "classId": "7.11.01"}], "name": "OEKOBAU.DAT"}, {"class": [{"value": "02 Bauprodukte", "level": 0}, {"value": "Fassaden", "level": 1}, {"value": "Sonnenschutzsysteme", "level": 2}], "name": "IBUCategories"}]}, "generalComment": [{"value": "Auenliegende Raffstoren sind auenliegende Sonnenschutzprodukte. Der Raffstore besteht aus horizontalen Lamellen. Die Lamellen sind seitlich in Fhrungsschienen eingehngt oder seilgefhrt und knnen vom Benutzer je nach Sonnenstand ausgerichtet werden. Der auenliegende Raffstore wird im eingefahrenen Zustand in einem Kastensystem verstaut. Das Produkt kann hand- oder kraftbetrieben sein. \nIm Sommer knnen auenliegende Raffstoren als Wrmeschutz eingesetzt werden. Bei diesem System wird die aus der Sonneneinstrahlung resultierende Absorptionswrme bereits vor den zu beschattenden Fensterteilen nach auen abgefhrt. Das Eindringen unerwnschter Sonnenwrme in das Gebudeinnere kann minimiert werden. Die jeweiligen Raffstoren knnen je nach Lamellenform eine fast vollstndige Verdunkelung erzielen. Dank der Einstellmglichkeiten lsst sich je nach Sonnenstand ein Gleichgewicht zwischen Lichtdurchlssigkeit, Tageslichtnutzung und Beschattung herstellen. Das verringert die berhitzung von Gebuden und minimiert die erforderliche Khlenergie sowie den Energieverbrauch fr knstliche Beleuchtung.", "lang": "de"}, {"value": "External Venetian blinds are external sunblind products. The blind consists of horizontal slats. The slats are mounted laterally in guide rails or guided by ropes and can be aligned by the user, depending on the position of the sun. The external Venetian blind is stowed in a box system when folded. The product can be operated manually or by power. \n\nThermal protection can be achieved in summer by using external Venetian blinds. With this system, the absorption heat resulting from the solar radiation is already dissipated externally in front of the window components to be shaded. The ingress of undesired solar heat in the building interior can be minimised. The respective blinds can achieve almost complete darkening depending on the slat shape. The setting options allow a balance to be established between transparency, daylight utilisation and shading, depending on the position of the sun. This reduces the overheating of buildings and minimises the cooling energy required and the energy used for artificial lighting.", "lang": "en"}]}, "quantitativeReference": {"referenceToReferenceFlow": [0]}, "time": {"referenceYear": 2024, "dataSetValidUntil": 2029, "other": {"anies": [{"name": "publicationDateOfEPD", "value": 1713225600000}]}}, "geography": {"locationOfOperationSupplyOrProduction": {"location": "RER"}}, "technology": {"technologyDescriptionAndIncludedProcesses": [{"value": "Sun protection systems are an assembly of several components. Process steps can include cutting, bending, stamping, drilling, foaming, coating, plastic injection moulding, plastic extrusion, assembling. 1 m² of the declared external venetian blind consists of the following materials in terms of percentage: Aluminium: 72% Steel: 16% PVC: 3% Metals (Others): 2% PA: 2% Others: 5% \nTechnische Daten: \nDie anwendbaren Daten beruhen auf der Leistungserklrung gem der BauPVO und den harmonisierten Normen auf Grundlage der Maschinenrichtlinie. \nLeistungswerte des Produkts gem der Leistungserklrung \n(BauPVO) in Bezug auf seine wesentlichen Merkmale gem EN 13659:2004+A1:2008. \nDeklarierte Einheit: \nDie deklarierte Einheit ist 1 m2 Sonnenschutzsystem nach den PCR. \nDie reprsentative Gre des Sonnenschutzes bezieht sich auf eine Standardfenstergre nach EN 14351-1 mit einer Flche von 1,82 m2 und einem Breiten-Hhen-Verhltnis von 1,23 m mal 1,48 m. Fr die Berechnung der kobilanz wurden Prozesse und Massen entsprechend von der reprsentativen Gre auf die deklarierte Einheit skaliert.", "lang": "de"}, {"value": "Sun protection systems are an assembly of several components. Process steps can include cutting, bending, stamping, drilling, foaming, coating, plastic injection moulding, plastic extrusion, assembling. 1 m² of the declared external venetian blind consists of the following materials in terms of percentage: Aluminium: 72% Steel: 16% PVC: 3% Metals (Others): 2% PA: 2% Others: 5% \nTechnical data: \nThe applicable data are based on the declaration of performance in accordance with the CPR and the harmonised standards based on the machinery directive.\nPerformance values of the product according to the declaration of performance (CPR) with regard to its essential features in accordance with EN 13659:2004+A1:2008. \nDeclared unit: \nThe declared unit is 1 m of sun protection system according to the PCR.\nThe representative size of the sun protection system refers to a standard window size according to EN 14351-1 with a surface of 1.82 m and a width-height ratio of 1.23 m by 1.48 m. For the calculation of the LCA, processes and masses were scaled accordingly from the representative size to the declared unit.", "lang": "en"}], "technologicalApplicability": [{"value": "Auenliegende Raffstoren sind auenliegende Sonnenschutzsysteme, die der Beschattung dienen. Die Verwendung dieser Produkte unterliegt den jeweiligen nationalen Vorschriften.", "lang": "de"}, {"value": "External Venetian blinds are external sunblind systems used for shading. The usage of these products is subject to the respective national regulations.", "lang": "en"}]}}, "modellingAndValidation": {"LCIMethodAndAllocation": {"typeOfDataSet": "EPD", "referenceToLCAMethodDetails": [{"shortDescription": [{"value": "Sonnenschutzsysteme.pdf", "lang": "de"}], "type": "source data set", "refObjectId": "e5b5cc92-144e-4405-bfd4-675a1c7033e3"}], "other": {"anies": [{"name": "subType", "value": "specific dataset"}]}}, "dataSourcesTreatmentAndRepresentativeness": {"referenceToDataSource": [{"shortDescription": [{"value": "GaBi Database (all versions)", "lang": "de"}], "type": "source data set", "refObjectId": "28d74cc0-db8b-4d7e-bc44-5f6d56ce0c4a"}, {"shortDescription": [{"value": "Sphera MLC (fka GaBi) CUP 2023.01", "lang": "de"}], "type": "source data set", "refObjectId": "6bcd5bfa-3623-48ab-a52b-6d5be8db82ed"}], "useAdviceForDataSet": [{"value": "Gültigkeitsbereich: \nIn dieser Verbands-EPD (Environmental Product Declaration bzw. UmweltProduktdeklaration) wird eine spezifische Produktkonfiguration auenliegender Raffstoren deklariert. Dieses System auenliegender Raffstoren wird von Herstellern produziert, die Mitglied der IVRSA sind. Die Daten basieren auf der Produktion in Mitteleuropa im Zeitraum 2020 - 2022. \nDie Daten wurden von 5 Unternehmen zur Verfgung gestellt, die einbaufertige Sonnenschutzsysteme herstellen (Alulux GmbH, Beck+Heun GmbH, REFLEXA-WERKE Albrecht GmbH, HELLA Sonnenschutztechnik GmbH und WAREMA Renkhoff SE). Weitere Daten wurden von Unternehmen zur Verfgung gestellt, die spezielle Teile und vorgefertigte Produkte herstellen (Somfy GmbH und VEKA AG). Die Konfiguration der Komponenten der auenliegenden Raffstoren basiert auf dem insgesamt meistverkauften/relevantesten Produkt. \nSystemgrenze: \nDeklarationstyp in Bezug auf die gem Abschnitt 5.2 der \nEN 15804+A2 abgedeckten Lebenszyklusstadien: Wiege bis Werkstor (Cradle to Gate) (A 1 - A3) mit den Optionen A4, A5, Modul B6, Module C1 - C4 und Modul D. \n\nModule A 1 bis A3: Diese Module bercksichtigen die Herstellung aller Systemkomponenten einschlielich der Bereitstellung aller Rohstoffe, Halbfabrikate und Energie sowie der Abfallbehandlung bis zum Ende der Abfalleigenschaft oder der Entsorgung von Produktionsabfllen. Die Auswirkungen des Verpackungsmaterials werden bercksichtigt. \n\nModul A4: Dieses Modul bercksichtigt den 100 km langen Transport zur Baustelle (Lkw-Transport, Diesel, EURO 6). Der Transportweg kann bei Bedarf durch lineare Skalierung der Ergebnisse der kobilanz von Modul A4 projektspezifisch angepasst werden. \n\nModul A5: Dieses Modul bercksichtigt die Behandlung von Verpackungsmaterial in der Einbauphase durch Energierckgewinnung. Thermische Behandlung in Hausmllverbrennungsanlagen (HMVA) unter der Annahme eines R1-Werts von> 0,6. Der Einbauaufwand wird nicht deklariert, da von einem manuellen Einbau ausgegangen wird. \n\nModul B6: \nBerechnung der Szenarien nach PCR Teil B: 20.000 Zyklen fr Raffstoren, wobei ein Zyklus ein einmaliges Kippen und Drehen umfasst. \n\nModul C1: Es wird davon ausgegangen, dass die Demontage des Produkts manuell erfolgt. Modul \nC1 werden daher keine Umweltauswirkungen zugeordnet.\n\nModul C2: Dieses Modul bercksichtigt den 50 km langen Transport zum Ort der Abfallbehandlung/Entsorgung (LkwTransport, Diesel, EURO 6). \n\nModul C3: Das Szenario zum Ende des Lebenswegs bercksichtigt das Recycling von Metallen, die nach der Demontage das Ende der Abfalleigenschaft erreichen. Es wird davon ausgegangen, dass Materialien mit einem Heizwert vor einem Verbrennungsprozess nicht das Ende der Abfalleigenschaft erreichen. Thermische Behandlung der Materialien in HMVA unter Annahme eines R1-Werts von> 0,6. Die Sammelquote wird auf 100 % festgesetzt. \n\nModul C4: Im Hinblick auf die Entsorgung wird in Modul C4 fr inerte Materialien ohne Heizwert (z. B. Glasfasern) ein europisches Szenario fr durchschnittliche Deponieemissionen deklariert. \nModul D: Modul D beinhaltet die Gutschriften aus dem Recycling und der Verbrennung von anfallenden Produktionsabfllen in Modul A3 sowie der Verbrennung von Verpackungsmaterialien in Modul A5 zusammen mit den Gutschriften durch recycelbare Materialien, die am Ende des Lebenszyklus anfallen, und den Gutschriften in Verbindung mit den Verbrennungsprozessen in Modul C3. Fr die thermische und elektrische Energie, die in den Modulen A3, A5 und C3 durch die thermische Behandlung von Produktions-, Verpackungs- und Produktabfllen erzeugt wird, wurden die vermiedenen Lasten durch die Umwandlung des Strommixes und der thermischen Energie aus Erdgas unter Verwendung europischer Datenstze berechnet. \n\nBetrachtungszeitraum \nDer Betrachtungszeitraum fr die Erhebung der Produktionsdaten und der daraus resultierenden Durchschnittswerte bezieht sich auf die Jahre 2020 - 2022.", "lang": "de"}, {"value": "Scope: \nIn this association EPD, a specific product configuration of external Venetian blinds is declared. This external Venetian blinds system is produced by manufacturers that are members of IVRSA. Data are based on production during 2020 – 2022 in Central Europe.\nData have been provided by 5 companies that produce ready-to-install sun protection systems (Alulux GmbH, Beck+Heun GmbH, REFLEXA-WERKE Albrecht GmbH, HELLA Sonnenschutztechnik GmbH and WAREMA Renkhoff SE). Additional data have been provided by companies producing specific parts and pre-fabricated products (Somfy GmbH and VEKA AG). The configuration of the external Venetian blinds components is based on the overall bestselling/ most relevant product. \nSystem boundary: \nDeclaration type with respect to life cycle stages covered according to clause 5.2 of EN 15804+A2: cradle to gate (A1-A3) with options A4, A5, module B6, modules C1–C4, and module D.\n\nModules A1 to A3: These modules consider the manufacturing of all system components including the provision of all raw materials, semi-finished products and energy, as well as waste processing up to the end-of-waste state or disposal of production waste that occur during manufacturing. The impact of packaging materials is included.\n\nModule A4: This module considers 100 km transport to the construction site (Truck transport, diesel, EURO 6) The transport distance can be modified project specific if required by linear scaling of the LCA results of module A4.\n\nModule A5: This module considers treatment of packaging material in the installation phase by energy recovery. Thermal treatment in municipal waste incineration (MWI) plants, assuming an R1 value of >0,6. Installation efforts are not declared as installation is assumed to be done manually.\n\nModule B6:\nCalculation of the scenarios according to the PCR Part B: 20,000 cycles for Venetian blinds, whereby a cycle comprises one-time tilting and turning.\n\nModule C1: It is assumed, that the deinstallation of the product is done manually. No environmental impacts are therefore assigned to module C1.\n\nModule C2: This module considers 50 km transport to the site of waste treatment/ disposal (Truck transport, diesel, EURO 6).\n\nModule C3: The end-of-life scenario considers the recycling of metals, which reach the end-of-waste status after de-installation. It is assumed that materials with a calorific value do not reach the end-of-waste status before an incineration process. Thermal treatment of materials in MWI plants, assuming an R1 value of >0,6. Collection rate is set to 100%.\n\nModule C4: Regarding disposal an European scenario for average landfill emissions is declared in module C4 for inert materials without a calorific value (e.g. glass fibre).\n\nModule D: Module D includes benefits from recycling and incineration of occurring production waste in module A3 and the incineration of packaging materials in module A5 along with benefits from recyclable materials that occur at the end-of-life and benefits related to the incineration processes in module C3. For the thermal and electrical energy generated in modules A3, A5 and C3 due to the thermal treatment of production, packaging and product waste, avoided burdens have been calculated by the inversion of electricity grid mix and thermal energy from natural gas, using European datasets.\n\nPeriod under review\nThe period under review for the collection of production data and resulting averages refers to 2020-2022.", "lang": "en"}], "other": {"anies": [{"name": "referenceToOriginalEPD", "value": {"shortDescription": {"value": "Außenliegender Raffstore.pdf", "defaultValue": "Außenliegender Raffstore.pdf", "lstrings": [{"lang": "de", "value": "Außenliegender Raffstore.pdf"}]}, "type": "source data set", "uuid": {"uuid": "225a37ea-0811-4564-8ce0-c23ccab9e2f5"}, "refObjectId": "225a37ea-0811-4564-8ce0-c23ccab9e2f5", "resourceURLs": ["https://oekobaudat.de/OEKOBAU.DAT/resource/sources/225a37ea-0811-4564-8ce0-c23ccab9e2f5/Aussenliegender_Raffstore_21909.pdf?version=00.01.000"]}}]}}, "validation": {"review": [{"referenceToNameOfReviewerAndInstitution": [{"shortDescription": [{"value": "Institut Bauen und Umwelt e. V.", "lang": "de"}], "type": "contact data set", "refObjectId": "d111dbec-b024-4be5-86c5-752d6eb2cf95", "uri": "../contacts/d111dbec-b024-4be5-86c5-752d6eb2cf95.xml"}], "type": "Accredited third party review"}]}, "complianceDeclarations": {"compliance": [{"referenceToComplianceSystem": {"shortDescription": [{"value": "DIN EN 15804+A2", "lang": "de"}], "type": "source data set", "refObjectId": "c0016b33-8cf7-415c-ac6e-deba0d21440d", "uri": "../sources/c0016b33-8cf7-415c-ac6e-deba0d21440d.xml"}}, {"referenceToComplianceSystem": {"shortDescription": [{"value": "ISO 14025", "lang": "de"}], "type": "source data set", "refObjectId": "4f2eb655-6e44-4874-a95a-e28f5442cd4d", "uri": "../sources/4f2eb655-6e44-4874-a95a-e28f5442cd4d.xml"}}]}}, "administrativeInformation": {"commissionerAndGoal": {"referenceToCommissioner": [{"shortDescription": [{"value": "IVRSA e.V.", "lang": "de"}], "type": "contact data set", "refObjectId": "0a3b4874-8639-4918-b7b3-20e3a9020730", "uri": "../contacts/0a3b4874-8639-4918-b7b3-20e3a9020730.xml"}]}, "dataGenerator": {"referenceToPersonOrEntityGeneratingTheDataSet": [{"shortDescription": [{"value": "Sphera Solutions GmbH", "lang": "de"}], "type": "contact data set", "refObjectId": "623edf96-39d1-4e6f-9892-674c7228546b", "uri": "../contacts/623edf96-39d1-4e6f-9892-674c7228546b.xml"}]}, "dataEntryBy": {"timeStamp": 1713225600000, "referenceToDataSetFormat": [{"shortDescription": [{"value": "ILCD Format", "lang": "de"}], "type": "source data set", "refObjectId": "a97a0155-0234-4b87-b4ce-a45da52f2a40", "uri": "../sources/a97a0155-0234-4b87-b4ce-a45da52f2a40.xml"}, {"shortDescription": [{"value": "EPD-Datenformaterweiterungen v1.2", "lang": "de"}, {"value": "EPD Data Format Extensions v1.2", "lang": "en"}], "type": "source data set", "refObjectId": "a29449fd-aa2f-4de8-b5d7-4b06b43c6fde", "uri": "../sources/a29449fd-aa2f-4de8-b5d7-4b06b43c6fde.xml"}]}, "publicationAndOwnership": {"dataSetVersion": "00.02.100", "referenceToRegistrationAuthority": {"shortDescription": [{"value": "Institut Bauen und Umwelt e. V.", "lang": "de"}], "type": "contact data set", "refObjectId": "d111dbec-b024-4be5-86c5-752d6eb2cf95", "uri": "../contacts/d111dbec-b024-4be5-86c5-752d6eb2cf95.xml"}, "registrationNumber": "EPD-IVR-20240103-CBA1-DE", "referenceToOwnershipOfDataSet": {"shortDescription": [{"value": "IVRSA e.V.", "lang": "de"}], "type": "contact data set", "refObjectId": "0a3b4874-8639-4918-b7b3-20e3a9020730", "uri": "../contacts/0a3b4874-8639-4918-b7b3-20e3a9020730.xml"}, "copyright": true, "licenseType": "Free of charge for all users and uses", "accessRestrictions": [{"value": "None", "lang": "en"}], "other": {"anies": [{"name": "referenceToPublisher", "value": {"shortDescription": [{"value": "Institut Bauen und Umwelt e. V.", "lang": "de"}], "type": "contact data set", "refObjectId": "d111dbec-b024-4be5-86c5-752d6eb2cf95", "uri": "../contacts/d111dbec-b024-4be5-86c5-752d6eb2cf95.xml"}}]}}}, "exchanges": {"exchange": [{"dataSetInternalID": 0, "referenceToFlowDataSet": {"shortDescription": [{"value": "External Venetian Blind (specific weight 7.84 kg/m²) (External Venetian Blind (specific weight 7.84 kg/m²))", "lang": "de"}], "type": "flow data set", "refObjectId": "a27e51e4-3673-8211-076e-d77458be7d0b", "uri": "../flows/a27e51e4-3673-8211-076e-d77458be7d0b.xml"}, "meanAmount": 1.0, "referencesToDataSource": {}, "referenceFlow": true, "resolvedFlowVersion": "00.02.100", "resultingflowAmount": 1.0, "flowProperties": [{"name": [{"lang": "de", "value": "Fläche"}, {"lang": "en", "value": "Area"}], "uuid": "93a60a56-a3c8-19da-a746-0800200c9a66", "referenceFlowProperty": true, "meanValue": 1.0, "referenceUnit": "qm", "unitGroupUUID": "c20a03d7-bd90-4569-bc94-66cfd364dfc8"}], "materialProperties": [{"name": "grammage", "value": "7.84", "unit": "kg/m^2", "unitDescription": "kilograms per square meter"}], "typeOfFlow": "Product flow", "classification": {"classHierarchy": "Komponenten von Fenstern und Vorhangfassaden / Zubehör für Fenster, Fassaden, Türen und Tore / Sonnenschutzsysteme", "name": "OEKOBAU.DAT"}}, {"dataSetInternalID": 1, "referenceToFlowDataSet": {"shortDescription": [{"value": "Erneuerbare Primärenergie als Energieträger (PERE)", "lang": "de"}, {"value": "Renewable primary energy as energy carrier (PERE)", "lang": "en"}], "type": "flow data set", "refObjectId": "20f32be5-0398-4288-9b6d-accddd195317", "uri": "../flows/20f32be5-0398-4288-9b6d-accddd195317.xml"}, "exchange direction": "INPUT", "other": {"anies": [{"name": "referenceToUnitGroupDataSet", "value": {"shortDescription": [{"value": "MJ", "lang": "de"}], "type": "unit group data set", "refObjectId": "93a60a57-a3c8-11da-a746-0800200c9a66", "uri": "../unitgroups/93a60a57-a3c8-11da-a746-0800200c9a66.xml"}}, {"value": "307.514953031721", "module": "A1-A3"}, {"value": "0.0647237996238085", "module": "A4"}, {"value": "15.1792787858852", "module": "A5"}, {"value": "19.5905635954252", "module": "B6"}, {"value": "0", "module": "C1"}, {"value": "0.0286272584839953", "module": "C2"}, {"value": "0.234472142384674", "module": "C3"}, {"value": "0.00145082834972552", "module": "C4"}, {"value": "-193.604031902768", "module": "D"}]}, "resolvedFlowVersion": "38.00.000", "flowProperties": [], "typeOfFlow": "Other flow", "classification": {"classHierarchy": "Quantities", "name": "GaBiCategories"}}, {"dataSetInternalID": 2, "referenceToFlowDataSet": {"shortDescription": [{"value": "Erneuerbare Primärenergie zur stofflichen Nutzung (PERM)", "lang": "de"}, {"value": "Renewable primary energy resources as material utilization (PERM)", "lang": "en"}], "type": "flow data set", "refObjectId": "fb3ec0de-548d-4508-aea5-00b73bf6f702", "uri": "../flows/fb3ec0de-548d-4508-aea5-00b73bf6f702.xml"}, "exchange direction": "INPUT", "other": {"anies": [{"name": "referenceToUnitGroupDataSet", "value": {"shortDescription": [{"value": "MJ", "lang": "de"}], "type": "unit group data set", "refObjectId": "93a60a57-a3c8-11da-a746-0800200c9a66", "uri": "../unitgroups/93a60a57-a3c8-11da-a746-0800200c9a66.xml"}}, {"value": "15.069744", "module": "A1-A3"}, {"value": "0", "module": "A4"}, {"value": "-15.069744", "module": "A5"}, {"value": "0", "module": "B6"}, {"value": "0", "module": "C1"}, {"value": "0", "module": "C2"}, {"value": "0", "module": "C3"}, {"value": "0", "module": "C4"}, {"value": "0", "module": "D"}]}, "resolvedFlowVersion": "38.00.000", "flowProperties": [], "typeOfFlow": "Other flow", "classification": {"classHierarchy": "Quantities", "name": "GaBiCategories"}}, {"dataSetInternalID": 3, "referenceToFlowDataSet": {"shortDescription": [{"value": "Total erneuerbare Primärenergie (PERT)", "lang": "de"}, {"value": "Total use of renewable primary energy resources (PERT)", "lang": "en"}], "type": "flow data set", "refObjectId": "53f97275-fa8a-4cdd-9024-65936002acd0", "uri": "../flows/53f97275-fa8a-4cdd-9024-65936002acd0.xml"}, "exchange direction": "INPUT", "other": {"anies": [{"name": "referenceToUnitGroupDataSet", "value": {"shortDescription": [{"value": "MJ", "lang": "de"}], "type": "unit group data set", "refObjectId": "93a60a57-a3c8-11da-a746-0800200c9a66", "uri": "../unitgroups/93a60a57-a3c8-11da-a746-0800200c9a66.xml"}}, {"value": "322.584697031721", "module": "A1-A3"}, {"value": "0.0647237996238085", "module": "A4"}, {"value": "0.109534785885159", "module": "A5"}, {"value": "19.5905635954252", "module": "B6"}, {"value": "0", "module": "C1"}, {"value": "0.0286272584839953", "module": "C2"}, {"value": "0.234472142384674", "module": "C3"}, {"value": "0.00145082834972552", "module": "C4"}, {"value": "-193.604031902768", "module": "D"}]}, "resolvedFlowVersion": "38.00.000", "flowProperties": [], "typeOfFlow": "Other flow", "classification": {"classHierarchy": "Quantities / Environmental quantities / EPD EN 15804 / LCI indicators", "name": "GaBiCategories"}}, {"dataSetInternalID": 4, "referenceToFlowDataSet": {"shortDescription": [{"value": "Nicht-erneuerbare Primärenergie als Energieträger (PENRE)", "lang": "de"}, {"value": "Non renewable primary energy as energy carrier (PENRE)", "lang": "en"}], "type": "flow data set", "refObjectId": "ac857178-2b45-46ec-892a-a9a4332f0372", "uri": "../flows/ac857178-2b45-46ec-892a-a9a4332f0372.xml"}, "exchange direction": "INPUT", "other": {"anies": [{"name": "referenceToUnitGroupDataSet", "value": {"shortDescription": [{"value": "MJ", "lang": "de"}], "type": "unit group data set", "refObjectId": "93a60a57-a3c8-11da-a746-0800200c9a66", "uri": "../unitgroups/93a60a57-a3c8-11da-a746-0800200c9a66.xml"}}, {"value": "897.227602386804", "module": "A1-A3"}, {"value": "0.892738717036563", "module": "A4"}, {"value": "7.09043916046407", "module": "A5"}, {"value": "143.016518615455", "module": "B6"}, {"value": "0", "module": "C1"}, {"value": "0.394857257451168", "module": "C2"}, {"value": "18.6600143850634", "module": "C3"}, {"value": "0.00890869866014845", "module": "C4"}, {"value": "-422.839146719625", "module": "D"}]}, "resolvedFlowVersion": "38.00.000", "flowProperties": [], "typeOfFlow": "Other flow", "classification": {"classHierarchy": "Quantities", "name": "GaBiCategories"}}, {"dataSetInternalID": 5, "referenceToFlowDataSet": {"shortDescription": [{"value": "Nicht-erneuerbare Primärenergie zur stofflichen Nutzung (PENRM)", "lang": "de"}, {"value": "Non renewable primary energy as material utilization (PENRM)", "lang": "en"}], "type": "flow data set", "refObjectId": "1421caa0-679d-4bf4-b282-0eb850ccae27", "uri": "../flows/1421caa0-679d-4bf4-b282-0eb850ccae27.xml"}, "exchange direction": "INPUT", "other": {"anies": [{"name": "referenceToUnitGroupDataSet", "value": {"shortDescription": [{"value": "MJ", "lang": "de"}], "type": "unit group data set", "refObjectId": "93a60a57-a3c8-11da-a746-0800200c9a66", "uri": "../unitgroups/93a60a57-a3c8-11da-a746-0800200c9a66.xml"}}, {"value": "24.2296", "module": "A1-A3"}, {"value": "0", "module": "A4"}, {"value": "-6.6066", "module": "A5"}, {"value": "0", "module": "B6"}, {"value": "0", "module": "C1"}, {"value": "0", "module": "C2"}, {"value": "-17.623", "module": "C3"}, {"value": "0", "module": "C4"}, {"value": "0", "module": "D"}]}, "resolvedFlowVersion": "38.00.000", "flowProperties": [], "typeOfFlow": "Other flow", "classification": {"classHierarchy": "Quantities", "name": "GaBiCategories"}}, {"dataSetInternalID": 6, "referenceToFlowDataSet": {"shortDescription": [{"value": "Total nicht erneuerbare Primärenergie (PENRT)", "lang": "de"}, {"value": "Total use of non renewable primary energy resources (PENRT)", "lang": "en"}], "type": "flow data set", "refObjectId": "06159210-646b-4c8d-8583-da9b3b95a6c1", "uri": "../flows/06159210-646b-4c8d-8583-da9b3b95a6c1.xml"}, "exchange direction": "INPUT", "other": {"anies": [{"name": "referenceToUnitGroupDataSet", "value": {"shortDescription": [{"value": "MJ", "lang": "de"}], "type": "unit group data set", "refObjectId": "93a60a57-a3c8-11da-a746-0800200c9a66", "uri": "../unitgroups/93a60a57-a3c8-11da-a746-0800200c9a66.xml"}}, {"value": "921.457202386806", "module": "A1-A3"}, {"value": "0.892738717036563", "module": "A4"}, {"value": "0.483839160464066", "module": "A5"}, {"value": "143.016518615455", "module": "B6"}, {"value": "0", "module": "C1"}, {"value": "0.394857257451168", "module": "C2"}, {"value": "1.03701438506337", "module": "C3"}, {"value": "0.00890869866014846", "module": "C4"}, {"value": "-422.839146719625", "module": "D"}]}, "resolvedFlowVersion": "38.00.000", "flowProperties": [], "typeOfFlow": "Other flow", "classification": {"classHierarchy": "Quantities / Environmental quantities / EPD EN 15804 / LCI indicators", "name": "GaBiCategories"}}, {"dataSetInternalID": 7, "referenceToFlowDataSet": {"shortDescription": [{"value": "Einsatz von Sekundärstoffen (SM)", "lang": "de"}, {"value": "Use of secondary material (SM)", "lang": "en"}], "type": "flow data set", "refObjectId": "c6a1f35f-2d09-4f54-8dfb-97e502e1ce92", "uri": "../flows/c6a1f35f-2d09-4f54-8dfb-97e502e1ce92.xml"}, "exchange direction": "INPUT", "other": {"anies": [{"name": "referenceToUnitGroupDataSet", "value": {"shortDescription": [{"value": "kg", "lang": "de"}], "type": "unit group data set", "refObjectId": "ad38d542-3fe9-439d-9b95-2f5f7752acaf", "uri": "../unitgroups/ad38d542-3fe9-439d-9b95-2f5f7752acaf.xml"}}, {"value": "2.37599069301848", "module": "A1-A3"}, {"value": "0", "module": "A4"}, {"value": "0", "module": "A5"}, {"value": "0", "module": "B6"}, {"value": "0", "module": "C1"}, {"value": "0", "module": "C2"}, {"value": "0", "module": "C3"}, {"value": "0", "module": "C4"}, {"value": "5.79435449427201", "module": "D"}]}, "resolvedFlowVersion": "38.00.000", "flowProperties": [], "typeOfFlow": "Other flow", "classification": {"classHierarchy": "Quantities / Environmental quantities / EPD EN 15804 / LCI indicators", "name": "GaBiCategories"}}, {"dataSetInternalID": 8, "referenceToFlowDataSet": {"shortDescription": [{"value": "Erneuerbare Sekundärbrennstoffe (RSF)", "lang": "de"}, {"value": "Use of renewable secondary fuels (RSF)", "lang": "en"}], "type": "flow data set", "refObjectId": "64333088-a55f-4aa2-9a31-c10b07816787", "uri": "../flows/64333088-a55f-4aa2-9a31-c10b07816787.xml"}, "exchange direction": "INPUT", "other": {"anies": [{"name": "referenceToUnitGroupDataSet", "value": {"shortDescription": [{"value": "MJ", "lang": "de"}], "type": "unit group data set", "refObjectId": "93a60a57-a3c8-11da-a746-0800200c9a66", "uri": "../unitgroups/93a60a57-a3c8-11da-a746-0800200c9a66.xml"}}, {"value": "0", "module": "A1-A3"}, {"value": "0", "module": "A4"}, {"value": "0", "module": "A5"}, {"value": "0", "module": "B6"}, {"value": "0", "module": "C1"}, {"value": "0", "module": "C2"}, {"value": "0", "module": "C3"}, {"value": "0", "module": "C4"}, {"value": "0", "module": "D"}]}, "resolvedFlowVersion": "38.00.000", "flowProperties": [], "typeOfFlow": "Other flow", "classification": {"classHierarchy": "Quantities / Environmental quantities / EPD EN 15804 / LCI indicators", "name": "GaBiCategories"}}, {"dataSetInternalID": 9, "referenceToFlowDataSet": {"shortDescription": [{"value": "Nicht erneuerbare Sekundärbrennstoffe (NRSF)", "lang": "de"}, {"value": "Use of non renewable secondary fuels (NRSF)", "lang": "en"}], "type": "flow data set", "refObjectId": "89def144-d39a-4287-b86f-efde453ddcb2", "uri": "../flows/89def144-d39a-4287-b86f-efde453ddcb2.xml"}, "exchange direction": "INPUT", "other": {"anies": [{"name": "referenceToUnitGroupDataSet", "value": {"shortDescription": [{"value": "MJ", "lang": "de"}], "type": "unit group data set", "refObjectId": "93a60a57-a3c8-11da-a746-0800200c9a66", "uri": "../unitgroups/93a60a57-a3c8-11da-a746-0800200c9a66.xml"}}, {"value": "0", "module": "A1-A3"}, {"value": "0", "module": "A4"}, {"value": "0", "module": "A5"}, {"value": "0", "module": "B6"}, {"value": "0", "module": "C1"}, {"value": "0", "module": "C2"}, {"value": "0", "module": "C3"}, {"value": "0", "module": "C4"}, {"value": "0", "module": "D"}]}, "resolvedFlowVersion": "38.00.000", "flowProperties": [], "typeOfFlow": "Other flow", "classification": {"classHierarchy": "Quantities / Environmental quantities / EPD EN 15804 / LCI indicators", "name": "GaBiCategories"}}, {"dataSetInternalID": 10, "referenceToFlowDataSet": {"shortDescription": [{"value": "Einsatz von Süßwasserressourcen (FW)", "lang": "de"}, {"value": "Use of net fresh water (FW)", "lang": "en"}], "type": "flow data set", "refObjectId": "3cf952c8-f3a4-461d-8c96-96456ca62246", "uri": "../flows/3cf952c8-f3a4-461d-8c96-96456ca62246.xml"}, "exchange direction": "INPUT", "other": {"anies": [{"name": "referenceToUnitGroupDataSet", "value": {"shortDescription": [{"value": "m^3", "lang": "de"}], "type": "unit group data set", "refObjectId": "cd950537-0a98-4044-9ba7-9f9a68d0a504", "uri": "../unitgroups/cd950537-0a98-4044-9ba7-9f9a68d0a504.xml"}}, {"value": "0.66210848372353", "module": "A1-A3"}, {"value": "7.08900047628655E-05", "module": "A4"}, {"value": "0.00456691397481217", "module": "A5"}, {"value": "0.0327844005317486", "module": "B6"}, {"value": "0", "module": "C1"}, {"value": "3.13545635774401E-05", "module": "C2"}, {"value": "0.00404586276078409", "module": "C3"}, {"value": "2.24901200749522E-06", "module": "C4"}, {"value": "-0.340380382635942", "module": "D"}]}, "resolvedFlowVersion": "38.00.000", "flowProperties": [], "typeOfFlow": "Other flow", "classification": {"classHierarchy": "Quantities / Environmental quantities / EPD EN 15804 / LCI indicators", "name": "GaBiCategories"}}, {"dataSetInternalID": 11, "referenceToFlowDataSet": {"shortDescription": [{"value": "Gefährlicher Abfall zur Deponie (HWD)", "lang": "de"}, {"value": "Hazardous waste disposed (HWD)", "lang": "en"}], "type": "flow data set", "refObjectId": "430f9e0f-59b2-46a0-8e0d-55e0e84948fc", "uri": "../flows/430f9e0f-59b2-46a0-8e0d-55e0e84948fc.xml"}, "exchange direction": "OUTPUT", "other": {"anies": [{"name": "referenceToUnitGroupDataSet", "value": {"shortDescription": [{"value": "kg", "lang": "de"}], "type": "unit group data set", "refObjectId": "ad38d542-3fe9-439d-9b95-2f5f7752acaf", "uri": "../unitgroups/ad38d542-3fe9-439d-9b95-2f5f7752acaf.xml"}}, {"value": "1.13078784891343E-06", "module": "A1-A3"}, {"value": "2.76420237921956E-12", "module": "A4"}, {"value": "1.25588383418764E-11", "module": "A5"}, {"value": "8.28949006020935E-09", "module": "B6"}, {"value": "0", "module": "C1"}, {"value": "1.22260337730365E-12", "module": "C2"}, {"value": "3.27495962500429E-11", "module": "C3"}, {"value": "1.93851899904265E-13", "module": "C4"}, {"value": "-1.80618359393667E-07", "module": "D"}]}, "resolvedFlowVersion": "38.00.000", "flowProperties": [], "typeOfFlow": "Other flow", "classification": {"classHierarchy": "Quantities / Environmental quantities / EPD EN 15804 / LCI indicators", "name": "GaBiCategories"}}, {"dataSetInternalID": 12, "referenceToFlowDataSet": {"shortDescription": [{"value": "Entsorgter nicht gefährlicher Abfall (NHWD)", "lang": "de"}, {"value": "Non hazardous waste disposed (NHWD)", "lang": "en"}], "type": "flow data set", "refObjectId": "b29ef66b-e286-4afa-949f-62f1a7b4d7fa", "uri": "../flows/b29ef66b-e286-4afa-949f-62f1a7b4d7fa.xml"}, "exchange direction": "OUTPUT", "other": {"anies": [{"name": "referenceToUnitGroupDataSet", "value": {"shortDescription": [{"value": "kg", "lang": "de"}], "type": "unit group data set", "refObjectId": "ad38d542-3fe9-439d-9b95-2f5f7752acaf", "uri": "../unitgroups/ad38d542-3fe9-439d-9b95-2f5f7752acaf.xml"}}, {"value": "14.1320418874162", "module": "A1-A3"}, {"value": "0.000136088329619802", "module": "A4"}, {"value": "0.0377859731681586", "module": "A5"}, {"value": "0.0315253762712179", "module": "B6"}, {"value": "0", "module": "C1"}, {"value": "6.01917039995308E-05", "module": "C2"}, {"value": "0.187069555574968", "module": "C3"}, {"value": "0.0445437322951523", "module": "C4"}, {"value": "-7.69044521272438", "module": "D"}]}, "resolvedFlowVersion": "38.00.000", "flowProperties": [], "typeOfFlow": "Other flow", "classification": {"classHierarchy": "Quantities / Environmental quantities / EPD EN 15804 / LCI indicators", "name": "GaBiCategories"}}, {"dataSetInternalID": 13, "referenceToFlowDataSet": {"shortDescription": [{"value": "Entsorgter radioaktiver Abfall (RWD)", "lang": "de"}, {"value": "Radioactive waste disposed (RWD)", "lang": "en"}], "type": "flow data set", "refObjectId": "3449546e-52ad-4b39-b809-9fb77cea8ff6", "uri": "../flows/3449546e-52ad-4b39-b809-9fb77cea8ff6.xml"}, "exchange direction": "OUTPUT", "other": {"anies": [{"name": "referenceToUnitGroupDataSet", "value": {"shortDescription": [{"value": "kg", "lang": "de"}], "type": "unit group data set", "refObjectId": "ad38d542-3fe9-439d-9b95-2f5f7752acaf", "uri": "../unitgroups/ad38d542-3fe9-439d-9b95-2f5f7752acaf.xml"}}, {"value": "0.0443984762854367", "module": "A1-A3"}, {"value": "1.67070741036191E-06", "module": "A4"}, {"value": "2.37099409355248E-05", "module": "A5"}, {"value": "0.0222788181889714", "module": "B6"}, {"value": "0", "module": "C1"}, {"value": "7.38951871885524E-07", "module": "C2"}, {"value": "3.06533138864502E-05", "module": "C3"}, {"value": "1.01571049127214E-07", "module": "C4"}, {"value": "-0.0458852224985152", "module": "D"}]}, "resolvedFlowVersion": "38.00.000", "flowProperties": [], "typeOfFlow": "Other flow", "classification": {"classHierarchy": "Quantities / Environmental quantities / EPD EN 15804 / LCI indicators", "name": "GaBiCategories"}}, {"dataSetInternalID": 14, "referenceToFlowDataSet": {"shortDescription": [{"value": "Komponenten für die Wiederverwendung (CRU)", "lang": "de"}, {"value": "Components for re-use (CRU)", "lang": "en"}], "type": "flow data set", "refObjectId": "a2b32f97-3fc7-4af2-b209-525bc6426f33", "uri": "../flows/a2b32f97-3fc7-4af2-b209-525bc6426f33.xml"}, "exchange direction": "OUTPUT", "other": {"anies": [{"name": "referenceToUnitGroupDataSet", "value": {"shortDescription": [{"value": "kg", "lang": "de"}], "type": "unit group data set", "refObjectId": "ad38d542-3fe9-439d-9b95-2f5f7752acaf", "uri": "../unitgroups/ad38d542-3fe9-439d-9b95-2f5f7752acaf.xml"}}, {"value": "0", "module": "A1-A3"}, {"value": "0", "module": "A4"}, {"value": "0", "module": "A5"}, {"value": "0", "module": "B6"}, {"value": "0", "module": "C1"}, {"value": "0", "module": "C2"}, {"value": "0", "module": "C3"}, {"value": "0", "module": "C4"}, {"value": "0", "module": "D"}]}, "resolvedFlowVersion": "38.00.000", "flowProperties": [], "typeOfFlow": "Other flow", "classification": {"classHierarchy": "Quantities / Environmental quantities / EPD EN 15804 / LCI indicators", "name": "GaBiCategories"}}, {"dataSetInternalID": 15, "referenceToFlowDataSet": {"shortDescription": [{"value": "Stoffe zum Recycling (MFR)", "lang": "de"}, {"value": "Materials for recycling (MFR)", "lang": "en"}], "type": "flow data set", "refObjectId": "d7fe48a5-4103-49c8-9aae-b0b5dfdbd6ae", "uri": "../flows/d7fe48a5-4103-49c8-9aae-b0b5dfdbd6ae.xml"}, "exchange direction": "OUTPUT", "other": {"anies": [{"name": "referenceToUnitGroupDataSet", "value": {"shortDescription": [{"value": "kg", "lang": "de"}], "type": "unit group data set", "refObjectId": "ad38d542-3fe9-439d-9b95-2f5f7752acaf", "uri": "../unitgroups/ad38d542-3fe9-439d-9b95-2f5f7752acaf.xml"}}, {"value": "0.544646590827797", "module": "A1-A3"}, {"value": "0", "module": "A4"}, {"value": "0", "module": "A5"}, {"value": "0", "module": "B6"}, {"value": "0", "module": "C1"}, {"value": "0", "module": "C2"}, {"value": "7.0033", "module": "C3"}, {"value": "0", "module": "C4"}, {"value": "0", "module": "D"}]}, "resolvedFlowVersion": "38.00.000", "flowProperties": [], "typeOfFlow": "Other flow", "classification": {"classHierarchy": "Quantities / Environmental quantities / EPD EN 15804 / LCI indicators", "name": "GaBiCategories"}}, {"dataSetInternalID": 16, "referenceToFlowDataSet": {"shortDescription": [{"value": "Stoffe für die Energierückgewinnung (MER)", "lang": "de"}, {"value": "Materials for energy recovery (MER)", "lang": "en"}], "type": "flow data set", "refObjectId": "59a9181c-3aaf-46ee-8b13-2b3723b6e447", "uri": "../flows/59a9181c-3aaf-46ee-8b13-2b3723b6e447.xml"}, "exchange direction": "OUTPUT", "other": {"anies": [{"name": "referenceToUnitGroupDataSet", "value": {"shortDescription": [{"value": "kg", "lang": "de"}], "type": "unit group data set", "refObjectId": "ad38d542-3fe9-439d-9b95-2f5f7752acaf", "uri": "../unitgroups/ad38d542-3fe9-439d-9b95-2f5f7752acaf.xml"}}, {"value": "0", "module": "A1-A3"}, {"value": "0", "module": "A4"}, {"value": "0", "module": "A5"}, {"value": "0", "module": "B6"}, {"value": "0", "module": "C1"}, {"value": "0", "module": "C2"}, {"value": "0", "module": "C3"}, {"value": "0", "module": "C4"}, {"value": "0", "module": "D"}]}, "resolvedFlowVersion": "38.00.000", "flowProperties": [], "typeOfFlow": "Other flow", "classification": {"classHierarchy": "Quantities / Environmental quantities / EPD EN 15804 / LCI indicators", "name": "GaBiCategories"}}, {"dataSetInternalID": 17, "referenceToFlowDataSet": {"shortDescription": [{"value": "Exportierte elektrische Energie (EEE)", "lang": "de"}, {"value": "Exported electrical energy (EEE)", "lang": "en"}], "type": "flow data set", "refObjectId": "4da0c987-2b76-40d6-9e9e-82a017aaaf29", "uri": "../flows/4da0c987-2b76-40d6-9e9e-82a017aaaf29.xml"}, "exchange direction": "OUTPUT", "other": {"anies": [{"name": "referenceToUnitGroupDataSet", "value": {"shortDescription": [{"value": "MJ", "lang": "de"}], "type": "unit group data set", "refObjectId": "93a60a57-a3c8-11da-a746-0800200c9a66", "uri": "../unitgroups/93a60a57-a3c8-11da-a746-0800200c9a66.xml"}}, {"value": "0", "module": "A1-A3"}, {"value": "0", "module": "A4"}, {"value": "1.43052708118692", "module": "A5"}, {"value": "0", "module": "B6"}, {"value": "0", "module": "C1"}, {"value": "0", "module": "C2"}, {"value": "2.02889438056979", "module": "C3"}, {"value": "0", "module": "C4"}, {"value": "0", "module": "D"}]}, "resolvedFlowVersion": "38.00.000", "flowProperties": [], "typeOfFlow": "Other flow", "classification": {"classHierarchy": "Quantities / Environmental quantities / EPD EN 15804 / LCI indicators", "name": "GaBiCategories"}}, {"dataSetInternalID": 18, "referenceToFlowDataSet": {"shortDescription": [{"value": "Exportierte thermische Energie (EET)", "lang": "de"}, {"value": "Exported thermal energy (EET)", "lang": "en"}], "type": "flow data set", "refObjectId": "98daf38a-7a79-46d3-9a37-2b7bd0955810", "uri": "../flows/98daf38a-7a79-46d3-9a37-2b7bd0955810.xml"}, "exchange direction": "OUTPUT", "other": {"anies": [{"name": "referenceToUnitGroupDataSet", "value": {"shortDescription": [{"value": "MJ", "lang": "de"}], "type": "unit group data set", "refObjectId": "93a60a57-a3c8-11da-a746-0800200c9a66", "uri": "../unitgroups/93a60a57-a3c8-11da-a746-0800200c9a66.xml"}}, {"value": "0", "module": "A1-A3"}, {"value": "0", "module": "A4"}, {"value": "2.55532129517394", "module": "A5"}, {"value": "0", "module": "B6"}, {"value": "0", "module": "C1"}, {"value": "0", "module": "C2"}, {"value": "3.80552874670212", "module": "C3"}, {"value": "0", "module": "C4"}, {"value": "0", "module": "D"}]}, "resolvedFlowVersion": "38.00.000", "flowProperties": [], "typeOfFlow": "Other flow", "classification": {"classHierarchy": "Quantities / Environmental quantities / EPD EN 15804 / LCI indicators", "name": "GaBiCategories"}}]}, "LCIAResults": {"LCIAResult": [{"referenceToLCIAMethodDataSet": {"shortDescription": [{"value": "Globales Erwärmungspotenzial total (GWP-total)", "lang": "de"}, {"value": "Global Warming Potential total (GWP-total)", "lang": "en"}], "type": "LCIA method data set", "refObjectId": "6a37f984-a4b3-458a-a20a-64418c145fa2", "uri": "../lciamethods/6a37f984-a4b3-458a-a20a-64418c145fa2.xml"}, "other": {"anies": [{"name": "referenceToUnitGroupDataSet", "value": {"shortDescription": [{"value": "kg CO_(2)-Äq.", "lang": "de"}], "type": "unit group data set", "refObjectId": "1ebf3012-d0db-4de2-aefd-ef30cedb0be1", "uri": "../unitgroups/1ebf3012-d0db-4de2-aefd-ef30cedb0be1.xml"}}, {"value": "62.6769553196389", "module": "A1-A3"}, {"value": "0.0660378710506203", "module": "A4"}, {"value": "1.8517332095515", "module": "A5"}, {"value": "6.51389268720758", "module": "B6"}, {"value": "0", "module": "C1"}, {"value": "0.0292084706906398", "module": "C2"}, {"value": "1.66026753993785", "module": "C3"}, {"value": "0.000670852701863324", "module": "C4"}, {"value": "-30.3975737302075", "module": "D"}]}}, {"referenceToLCIAMethodDataSet": {"shortDescription": [{"value": "Globales Erwärmungspotenzial fossil (GWP-fossil)", "lang": "de"}, {"value": "Global Warming Potential fossil fuels (GWP-fossil)", "lang": "en"}], "type": "LCIA method data set", "refObjectId": "5f635281-343e-44fb-83df-1971b155e6b6", "uri": "../lciamethods/5f635281-343e-44fb-83df-1971b155e6b6.xml"}, "other": {"anies": [{"name": "referenceToUnitGroupDataSet", "value": {"shortDescription": [{"value": "kg CO_(2)-Äq.", "lang": "de"}], "type": "unit group data set", "refObjectId": "1ebf3012-d0db-4de2-aefd-ef30cedb0be1", "uri": "../unitgroups/1ebf3012-d0db-4de2-aefd-ef30cedb0be1.xml"}}, {"value": "63.9324491763278", "module": "A1-A3"}, {"value": "0.0652404226997207", "module": "A4"}, {"value": "0.491705765445541", "module": "A5"}, {"value": "6.51005665827357", "module": "B6"}, {"value": "0", "module": "C1"}, {"value": "0.0288557602471627", "module": "C2"}, {"value": "1.66003905656935", "module": "C3"}, {"value": "0.000668775812931793", "module": "C4"}, {"value": "-30.3046425967012", "module": "D"}]}}, {"referenceToLCIAMethodDataSet": {"shortDescription": [{"value": "Globales Erwärmungspotenzial biogen (GWP-biogenic)", "lang": "de"}, {"value": "Global Warming Potential biogenic (GWP-biogenic)", "lang": "en"}], "type": "LCIA method data set", "refObjectId": "2356e1ab-0185-4db5-86e5-16de51c7485c", "uri": "../lciamethods/2356e1ab-0185-4db5-86e5-16de51c7485c.xml"}, "other": {"anies": [{"name": "referenceToUnitGroupDataSet", "value": {"shortDescription": [{"value": "kg CO_(2)-Äq.", "lang": "de"}], "type": "unit group data set", "refObjectId": "1ebf3012-d0db-4de2-aefd-ef30cedb0be1", "uri": "../unitgroups/1ebf3012-d0db-4de2-aefd-ef30cedb0be1.xml"}}, {"value": "-1.28702124991948", "module": "A1-A3"}, {"value": "0.00019279526016004", "module": "A4"}, {"value": "1.35998562115695", "module": "A5"}, {"value": "0.00324058824423812", "module": "B6"}, {"value": "0", "module": "C1"}, {"value": "8.52731109602591E-05", "module": "C2"}, {"value": "0.000193132170671404", "module": "C3"}, {"value": "0", "module": "C4"}, {"value": "-0.0869799614843552", "module": "D"}]}}, {"referenceToLCIAMethodDataSet": {"shortDescription": [{"value": "Globales Erwärmungspotenzial luluc (GWP-luluc)", "lang": "de"}, {"value": "Global Warming Potential luluc (GWP-luluc)", "lang": "en"}], "type": "LCIA method data set", "refObjectId": "4331bbdb-978a-490d-8707-eeb047f01a55", "uri": "../lciamethods/4331bbdb-978a-490d-8707-eeb047f01a55.xml"}, "other": {"anies": [{"name": "referenceToUnitGroupDataSet", "value": {"shortDescription": [{"value": "kg CO_(2)-Äq.", "lang": "de"}], "type": "unit group data set", "refObjectId": "1ebf3012-d0db-4de2-aefd-ef30cedb0be1", "uri": "../unitgroups/1ebf3012-d0db-4de2-aefd-ef30cedb0be1.xml"}}, {"value": "0.0315273932306206", "module": "A1-A3"}, {"value": "0.000604653090739534", "module": "A4"}, {"value": "4.18229490057057E-05", "module": "A5"}, {"value": "0.000595440689772237", "module": "B6"}, {"value": "0", "module": "C1"}, {"value": "0.000267437332516863", "module": "C2"}, {"value": "3.5351197830498E-05", "module": "C3"}, {"value": "2.07688893153075E-06", "module": "C4"}, {"value": "-0.00595117202186601", "module": "D"}]}}, {"referenceToLCIAMethodDataSet": {"shortDescription": [{"value": "Abbau Potential der stratosphärischen Ozonschicht (ODP)", "lang": "de"}, {"value": "Depletion potential of the stratospheric ozone layer (ODP)", "lang": "en"}], "type": "LCIA method data set", "refObjectId": "b5c629d6-def3-11e6-bf01-fe55135034f3", "uri": "../lciamethods/b5c629d6-def3-11e6-bf01-fe55135034f3.xml"}, "other": {"anies": [{"name": "referenceToUnitGroupDataSet", "value": {"shortDescription": [{"value": "kg CFC11-Äq.", "lang": "de"}], "type": "unit group data set", "refObjectId": "d9e957c9-7309-4474-bf3a-7777df6c4e5b", "uri": "../unitgroups/d9e957c9-7309-4474-bf3a-7777df6c4e5b.xml"}}, {"value": "1.50524931150035E-10", "module": "A1-A3"}, {"value": "8.49497121734745E-15", "module": "A4"}, {"value": "1.6941736648212E-13", "module": "A5"}, {"value": "6.40185048741653E-11", "module": "B6"}, {"value": "0", "module": "C1"}, {"value": "3.75731552020394E-15", "module": "C2"}, {"value": "4.44721506221735E-13", "module": "C3"}, {"value": "1.70034076877985E-15", "module": "C4"}, {"value": "-2.27319589453583E-10", "module": "D"}]}}, {"referenceToLCIAMethodDataSet": {"shortDescription": [{"value": "Versauerungspotenzial von Boden und Wasser (AP)", "lang": "de"}, {"value": "Acidification potential of land and water (AP)", "lang": "en"}], "type": "LCIA method data set", "refObjectId": "b5c611c6-def3-11e6-bf01-fe55135034f3", "uri": "../lciamethods/b5c611c6-def3-11e6-bf01-fe55135034f3.xml"}, "other": {"anies": [{"name": "referenceToUnitGroupDataSet", "value": {"shortDescription": [{"value": "mol H^(+)-Äq.", "lang": "de"}], "type": "unit group data set", "refObjectId": "42e089ac-92bf-4bf2-8ca1-5fc40d18f2ed", "uri": "../unitgroups/42e089ac-92bf-4bf2-8ca1-5fc40d18f2ed.xml"}}, {"value": "0.240616531912566", "module": "A1-A3"}, {"value": "8.64691666275118E-05", "module": "A4"}, {"value": "0.000361262260649243", "module": "A5"}, {"value": "0.00991462449331565", "module": "B6"}, {"value": "0", "module": "C1"}, {"value": "3.824520807383E-05", "module": "C2"}, {"value": "0.000967948910478335", "module": "C3"}, {"value": "4.74132205672213E-06", "module": "C4"}, {"value": "-0.115949653361195", "module": "D"}]}}, {"referenceToLCIAMethodDataSet": {"shortDescription": [{"value": "Eutrophierungspotenzial Süßwasser (EP-freshwater)", "lang": "de"}, {"value": "Eutrophication potential aquatic freshwater (EP-freshwater)", "lang": "en"}], "type": "LCIA method data set", "refObjectId": "b53ec18f-7377-4ad3-86eb-cc3f4f276b2b", "uri": "../lciamethods/b53ec18f-7377-4ad3-86eb-cc3f4f276b2b.xml"}, "other": {"anies": [{"name": "referenceToUnitGroupDataSet", "value": {"shortDescription": [{"value": "kg P-Äq.", "lang": "de"}], "type": "unit group data set", "refObjectId": "0429039d-a61d-4590-ba67-aa4a20a810a1", "uri": "../unitgroups/0429039d-a61d-4590-ba67-aa4a20a810a1.xml"}}, {"value": "0.000110100383047087", "module": "A1-A3"}, {"value": "2.38696966595477E-07", "module": "A4"}, {"value": "6.40065397249152E-08", "module": "A5"}, {"value": "6.43540188815517E-06", "module": "B6"}, {"value": "0", "module": "C1"}, {"value": "1.05575380335995E-07", "module": "C2"}, {"value": "1.29249125831731E-07", "module": "C3"}, {"value": "1.3461414010316E-09", "module": "C4"}, {"value": "-1.53806293697979E-05", "module": "D"}]}}, {"referenceToLCIAMethodDataSet": {"shortDescription": [{"value": "Eutrophierungspotenzial Salzwasser (EP-marine)", "lang": "de"}, {"value": "Eutrophication potential aquatic marine (EP-marine)", "lang": "en"}], "type": "LCIA method data set", "refObjectId": "b5c619fa-def3-11e6-bf01-fe55135034f3", "uri": "../lciamethods/b5c619fa-def3-11e6-bf01-fe55135034f3.xml"}, "other": {"anies": [{"name": "referenceToUnitGroupDataSet", "value": {"shortDescription": [{"value": "kg N-Äq.", "lang": "de"}], "type": "unit group data set", "refObjectId": "d05bb823-ecdf-4686-8c40-bf1d9257859f", "uri": "../unitgroups/d05bb823-ecdf-4686-8c40-bf1d9257859f.xml"}}, {"value": "0.043018510128202", "module": "A1-A3"}, {"value": "2.9836850864788E-05", "module": "A4"}, {"value": "0.000120429587076748", "module": "A5"}, {"value": "0.00279540378751825", "module": "B6"}, {"value": "0", "module": "C1"}, {"value": "1.31968031391733E-05", "module": "C2"}, {"value": "0.000438422004716291", "module": "C3"}, {"value": "1.22508295719278E-06", "module": "C4"}, {"value": "-0.0152811360573288", "module": "D"}]}}, {"referenceToLCIAMethodDataSet": {"shortDescription": [{"value": "Eutrophierungspotenzial Land (EP-terrestrial)", "lang": "de"}, {"value": "Eutrophication potential terrestrial (EP-terrestrial)", "lang": "en"}], "type": "LCIA method data set", "refObjectId": "b5c614d2-def3-11e6-bf01-fe55135034f3", "uri": "../lciamethods/b5c614d2-def3-11e6-bf01-fe55135034f3.xml"}, "other": {"anies": [{"name": "referenceToUnitGroupDataSet", "value": {"shortDescription": [{"value": "mol N-Äq.", "lang": "de"}], "type": "unit group data set", "refObjectId": "71b4d617-0ec9-4d3f-b65e-e438940c2401", "uri": "../unitgroups/71b4d617-0ec9-4d3f-b65e-e438940c2401.xml"}}, {"value": "0.46315077015393", "module": "A1-A3"}, {"value": "0.000357206081163898", "module": "A4"}, {"value": "0.00162595990788918", "module": "A5"}, {"value": "0.0295286817949332", "module": "B6"}, {"value": "0", "module": "C1"}, {"value": "0.000157991818727718", "module": "C2"}, {"value": "0.0051974853896347", "module": "C3"}, {"value": "1.34789714326925E-05", "module": "C4"}, {"value": "-0.165852084452308", "module": "D"}]}}, {"referenceToLCIAMethodDataSet": {"shortDescription": [{"value": "Bildungspotential für troposphärisches Ozon (POCP)", "lang": "de"}, {"value": "Formation potential of tropospheric ozone photochemical oxidants (POCP)", "lang": "en"}], "type": "LCIA method data set", "refObjectId": "b5c610fe-def3-11e6-bf01-fe55135034f3", "uri": "../lciamethods/b5c610fe-def3-11e6-bf01-fe55135034f3.xml"}, "other": {"anies": [{"name": "referenceToUnitGroupDataSet", "value": {"shortDescription": [{"value": "kg NMVOC-Äq.", "lang": "de"}], "type": "unit group data set", "refObjectId": "d27c25f8-fbc1-44c6-b47b-4adbae4199c6", "uri": "../unitgroups/d27c25f8-fbc1-44c6-b47b-4adbae4199c6.xml"}}, {"value": "0.194685404177744", "module": "A1-A3"}, {"value": "7.4953703290188E-05", "module": "A4"}, {"value": "0.000323027155720134", "module": "A5"}, {"value": "0.00772597407683621", "module": "B6"}, {"value": "0", "module": "C1"}, {"value": "3.31519325332006E-05", "module": "C2"}, {"value": "0.00113140870400375", "module": "C3"}, {"value": "3.69679087259567E-06", "module": "C4"}, {"value": "-0.0483872791751011", "module": "D"}]}}, {"referenceToLCIAMethodDataSet": {"shortDescription": [{"value": "Potenzial für den abiotischen Abbau nicht fossiler Ressourcen (ADPE)", "lang": "de"}, {"value": "Abiotic depletion potential for non fossil resources (ADPE)", "lang": "en"}], "type": "LCIA method data set", "refObjectId": "b2ad6494-c78d-11e6-9d9d-cec0c932ce01", "uri": "../lciamethods/b2ad6494-c78d-11e6-9d9d-cec0c932ce01.xml"}, "other": {"anies": [{"name": "referenceToUnitGroupDataSet", "value": {"shortDescription": [{"value": "kg Sb-Äq.", "lang": "de"}], "type": "unit group data set", "refObjectId": "54ccd2d9-a32a-4fc2-923d-f2c8c93e89d4", "uri": "../unitgroups/54ccd2d9-a32a-4fc2-923d-f2c8c93e89d4.xml"}}, {"value": "0.000452258147021513", "module": "A1-A3"}, {"value": "4.29965482069136E-09", "module": "A4"}, {"value": "1.80154141809517E-09", "module": "A5"}, {"value": "3.15284069555349E-07", "module": "B6"}, {"value": "0", "module": "C1"}, {"value": "1.90173213963493E-09", "module": "C2"}, {"value": "3.85036856224468E-09", "module": "C3"}, {"value": "3.08188057527596E-11", "module": "C4"}, {"value": "-0.000291741275266752", "module": "D"}]}}, {"referenceToLCIAMethodDataSet": {"shortDescription": [{"value": "Potenzial für den abiotischen Abbau fossiler Brennstoffe (ADPF)", "lang": "de"}, {"value": "Abiotic depletion potential for fossil resources (ADPF)", "lang": "en"}], "type": "LCIA method data set", "refObjectId": "b2ad6110-c78d-11e6-9d9d-cec0c932ce01", "uri": "../lciamethods/b2ad6110-c78d-11e6-9d9d-cec0c932ce01.xml"}, "other": {"anies": [{"name": "referenceToUnitGroupDataSet", "value": {"shortDescription": [{"value": "MJ", "lang": "de"}], "type": "unit group data set", "refObjectId": "93a60a57-a3c8-11da-a746-0800200c9a66", "uri": "../unitgroups/93a60a57-a3c8-11da-a746-0800200c9a66.xml"}}, {"value": "919.906601901276", "module": "A1-A3"}, {"value": "0.889373928623063", "module": "A4"}, {"value": "0.483328077721757", "module": "A5"}, {"value": "142.991208574537", "module": "B6"}, {"value": "0", "module": "C1"}, {"value": "0.393369015595512", "module": "C2"}, {"value": "1.03664048258664", "module": "C3"}, {"value": "0.0088986660114033", "module": "C4"}, {"value": "-422.50935514647", "module": "D"}]}}, {"referenceToLCIAMethodDataSet": {"shortDescription": [{"value": "Wassernutzung (WDP)", "lang": "de"}, {"value": "Water use (WDP)", "lang": "en"}], "type": "LCIA method data set", "refObjectId": "b2ad66ce-c78d-11e6-9d9d-cec0c932ce01", "uri": "../lciamethods/b2ad66ce-c78d-11e6-9d9d-cec0c932ce01.xml"}, "other": {"anies": [{"name": "referenceToUnitGroupDataSet", "value": {"shortDescription": [{"value": "m^(3) Welt-Äq. entzogen", "lang": "de"}], "type": "unit group data set", "refObjectId": "6ae2df01-888e-46c8-b17d-49fa3869b476", "uri": "../unitgroups/6ae2df01-888e-46c8-b17d-49fa3869b476.xml"}}, {"value": "7.4435266852823", "module": "A1-A3"}, {"value": "0.000788914181959421", "module": "A4"}, {"value": "0.194096352385598", "module": "A5"}, {"value": "0.547075315010915", "module": "B6"}, {"value": "0", "module": "C1"}, {"value": "0.00034893579085141", "module": "C2"}, {"value": "0.169150180398857", "module": "C3"}, {"value": "7.33952232065921E-05", "module": "C4"}, {"value": "-1.47668241410383", "module": "D"}]}}, {"referenceToLCIAMethodDataSet": {"shortDescription": [{"value": "Auftreten von Krankheiten aufgrund von Feinstaubemissionen (PM)", "lang": "de"}, {"value": "Incidence of disease due to PM emissions (PM)", "lang": "en"}], "type": "LCIA method data set", "refObjectId": "b5c602c6-def3-11e6-bf01-fe55135034f3", "uri": "../lciamethods/b5c602c6-def3-11e6-bf01-fe55135034f3.xml"}, "other": {"anies": [{"name": "referenceToUnitGroupDataSet", "value": {"shortDescription": [{"value": "Krankheitsfälle", "lang": "de"}], "type": "unit group data set", "refObjectId": "3883559b-648f-4afc-8ba2-0bd24f3affa3", "uri": "../unitgroups/3883559b-648f-4afc-8ba2-0bd24f3affa3.xml"}}, {"value": "2.649446584456E-06", "module": "A1-A3"}, {"value": "6.2394490405087E-10", "module": "A4"}, {"value": "2.0694542509515E-09", "module": "A5"}, {"value": "8.96376105640476E-08", "module": "B6"}, {"value": "0", "module": "C1"}, {"value": "2.75970078268789E-10", "module": "C2"}, {"value": "4.77795313989391E-09", "module": "C3"}, {"value": "5.83149598170161E-11", "module": "C4"}, {"value": "-1.82624094445677E-06", "module": "D"}]}}, {"referenceToLCIAMethodDataSet": {"shortDescription": [{"value": "Wirkung durch Exposition des Menschen mit U235 (IR)", "lang": "de"}, {"value": "Human exposure efficiency relative to U235 (IR)", "lang": "en"}], "type": "LCIA method data set", "refObjectId": "b5c632be-def3-11e6-bf01-fe55135034f3", "uri": "../lciamethods/b5c632be-def3-11e6-bf01-fe55135034f3.xml"}, "other": {"anies": [{"name": "referenceToUnitGroupDataSet", "value": {"shortDescription": [{"value": "kBq U235-Äq.", "lang": "de"}], "type": "unit group data set", "refObjectId": "456b05bf-1415-44a9-9993-02452f554c09", "uri": "../unitgroups/456b05bf-1415-44a9-9993-02452f554c09.xml"}}, {"value": "8.14276201374613", "module": "A1-A3"}, {"value": "0.000249145899086945", "module": "A4"}, {"value": "0.0037752778640977", "module": "A5"}, {"value": "3.3451754465456", "module": "B6"}, {"value": "0", "module": "C1"}, {"value": "0.000110196930570278", "module": "C2"}, {"value": "0.00392555478138954", "module": "C3"}, {"value": "1.17354995650979E-05", "module": "C4"}, {"value": "-9.3021163027022", "module": "D"}]}}, {"referenceToLCIAMethodDataSet": {"shortDescription": [{"value": "Toxizitätsvergleichseinheit für Ökosysteme (ETP-fw)", "lang": "de"}, {"value": "Comparative toxic unit for ecosystems (ETP-fw)", "lang": "en"}], "type": "LCIA method data set", "refObjectId": "ee1082d1-b0f7-43ca-a1f0-21e2a4a74511", "uri": "../lciamethods/ee1082d1-b0f7-43ca-a1f0-21e2a4a74511.xml"}, "other": {"anies": [{"name": "referenceToUnitGroupDataSet", "value": {"shortDescription": [{"value": "CTUe", "lang": "de"}], "type": "unit group data set", "refObjectId": "aa959ded-f1eb-4efb-9c5c-2d60be36b3e6", "uri": "../unitgroups/aa959ded-f1eb-4efb-9c5c-2d60be36b3e6.xml"}}, {"value": "344.19020203338", "module": "A1-A3"}, {"value": "0.631681021117191", "module": "A4"}, {"value": "0.239027531201919", "module": "A5"}, {"value": "40.9556559235213", "module": "B6"}, {"value": "0", "module": "C1"}, {"value": "0.279391753513556", "module": "C2"}, {"value": "0.545884498969106", "module": "C3"}, {"value": "0.00485702024396316", "module": "C4"}, {"value": "-159.235249734704", "module": "D"}]}}, {"referenceToLCIAMethodDataSet": {"shortDescription": [{"value": "Toxizitätsvergleichseinheit für Menschen (krebserregend) (HTP-c)", "lang": "de"}, {"value": "Comparative toxic unit for humans (carcinogenic) (HTP-c)", "lang": "en"}], "type": "LCIA method data set", "refObjectId": "2299222a-bbd8-474f-9d4f-4dd1f18aea7c", "uri": "../lciamethods/2299222a-bbd8-474f-9d4f-4dd1f18aea7c.xml"}, "other": {"anies": [{"name": "referenceToUnitGroupDataSet", "value": {"shortDescription": [{"value": "CTUh", "lang": "de"}], "type": "unit group data set", "refObjectId": "d4c9523e-2d7e-49fd-8469-998f547d3a70", "uri": "../unitgroups/d4c9523e-2d7e-49fd-8469-998f547d3a70.xml"}}, {"value": "4.99940251164286E-08", "module": "A1-A3"}, {"value": "1.2926075361276E-11", "module": "A4"}, {"value": "1.49202968703365E-11", "module": "A5"}, {"value": "7.38916727628658E-10", "module": "B6"}, {"value": "0", "module": "C1"}, {"value": "5.71718753691238E-12", "module": "C2"}, {"value": "2.88218446640312E-11", "module": "C3"}, {"value": "7.47619370391734E-13", "module": "C4"}, {"value": "-1.0550163261834E-08", "module": "D"}]}}, {"referenceToLCIAMethodDataSet": {"shortDescription": [{"value": "Toxizitätsvergleichseinheit für Menschen (nicht krebserregend) (HTP-nc)", "lang": "de"}, {"value": "Comparative toxic unit for humans (noncarcinogenic) (HTP-nc)", "lang": "en"}], "type": "LCIA method data set", "refObjectId": "3af763a5-b7a1-48c9-9cee-1f223481fcef", "uri": "../lciamethods/3af763a5-b7a1-48c9-9cee-1f223481fcef.xml"}, "other": {"anies": [{"name": "referenceToUnitGroupDataSet", "value": {"shortDescription": [{"value": "CTUh", "lang": "de"}], "type": "unit group data set", "refObjectId": "d4c9523e-2d7e-49fd-8469-998f547d3a70", "uri": "../unitgroups/d4c9523e-2d7e-49fd-8469-998f547d3a70.xml"}}, {"value": "1.00190552143087E-06", "module": "A1-A3"}, {"value": "6.88493083949245E-10", "module": "A4"}, {"value": "6.74435034136664E-10", "module": "A5"}, {"value": "3.7823633944814E-08", "module": "B6"}, {"value": "0", "module": "C1"}, {"value": "3.04519660360112E-10", "module": "C2"}, {"value": "2.21235220599121E-09", "module": "C3"}, {"value": "8.22269420924055E-11", "module": "C4"}, {"value": "-1.6927514414458E-07", "module": "D"}]}}, {"referenceToLCIAMethodDataSet": {"shortDescription": [{"value": "Bodenqualitätsindex (SQP)", "lang": "de"}, {"value": "Soil quality index (SQP)", "lang": "en"}], "type": "LCIA method data set", "refObjectId": "b2ad6890-c78d-11e6-9d9d-cec0c932ce01", "uri": "../lciamethods/b2ad6890-c78d-11e6-9d9d-cec0c932ce01.xml"}, "other": {"anies": [{"name": "referenceToUnitGroupDataSet", "value": {"shortDescription": [{"value": "SQP", "lang": "de"}], "type": "unit group data set", "refObjectId": "f130951c-e67f-4f7f-8dd4-665de3974e18", "uri": "../unitgroups/f130951c-e67f-4f7f-8dd4-665de3974e18.xml"}}, {"value": "235.830921927469", "module": "A1-A3"}, {"value": "0.37161623451861", "module": "A4"}, {"value": "0.149529910761263", "module": "A5"}, {"value": "19.3478626587663", "module": "B6"}, {"value": "0", "module": "C1"}, {"value": "0.164365412170582", "module": "C2"}, {"value": "0.227113149081839", "module": "C3"}, {"value": "0.00216192223758432", "module": "C4"}, {"value": "-15.0306766968595", "module": "D"}]}}]}, "otherAttributes": {"{http://www.indata.network/EPD/2019}epd-version": "1.2"}, "version": "1.1", "locations": "../ILCDLocations.xml"}