{"processInformation": {"dataSetInformation": {"UUID": "6cec8612-c5c4-4ea9-89f8-38f31ee36c66", "name": {"baseName": [{"value": "noraplan® 913 3 mm", "lang": "de"}, {"value": "noraplan® 913 3 mm", "lang": "en"}], "functionalUnitFlowProperties": [{"lang": "de"}]}, "classificationInformation": {"classification": [{"class": [{"value": "Kunststoffe", "level": 0, "classId": "6"}, {"value": "Bodenbeläge", "level": 1, "classId": "6.2"}, {"value": "Gummi-/Kautschuk-Bodenbeläge", "level": 2, "classId": "6.2.02"}], "name": "OEKOBAU.DAT"}, {"class": [{"value": "02 Bauprodukte", "level": 0}, {"value": "Bodenbeläge", "level": 1}, {"value": "Bodenbeläge", "level": 2}], "name": "IBUCategories"}]}, "generalComment": [{"value": "In dieser Umwelt-Produktdeklaration (EPD) werden rezepturgleiche elastische Kautschuk-Bodenbelge der Produktfamilie noraplan® 913 mit verschiedenen Designs und Oberflchenstrukturen der nora systems GmbH abgebildet.\nBesondere Merkmale der noraplan® 913 Belge sind:\n\nKontinuierlich vulkanisierte Kautschukbelge in Bahnen\n\nBelagsaufbau: Einschichtig\nOhne Zusatz von PVC, chlorhaltigen Polymeren und Phthalat-Weichmachern\nDauerelastische Eigenschaften\nGeeignet fr hchste Beanspruchungen\nKeine Beschichtungen bentigt\n\nErhhte Sicherheit wegen hoher Brandschutzeigenschaften \nUnverfugte Verlegung\nHohe Bestndigkeit gegen Chemikalien und Flchen- sowie Handdesinfektionsmittel gem den Listen von VAH und RKI", "lang": "de"}, {"value": "This Environmental Product Declaration (EPD) covers elastomeric rubber floor coverings of the noraplan® 913 product family with identical formulations but various designs and surface structures from nora systems GmbH.\nSpecial features of the noraplan® 913 coverings are:\n\nContinuously vulcanized rubber coverings in sheets\n\nCovering structure: Single-layer\nWithout addition of PVC, chlorine-containing polymers and phthalate plasticizers\nPermanently elastic properties\nSuitable for highest stress loads\nNo coatings required\n\nEnhanced safety due to high fire protection properties\nSeamless installation\nHigh resistance to chemicals and surface as well as hand disinfectants according to VAH and RKI lists", "lang": "en"}]}, "quantitativeReference": {"referenceToReferenceFlow": [0]}, "time": {"referenceYear": 2024, "dataSetValidUntil": 2029, "other": {"anies": [{"name": "publicationDateOfEPD", "value": 1733356800000}]}}, "geography": {"locationOfOperationSupplyOrProduction": {"location": "RER"}}, "technology": {"technologyDescriptionAndIncludedProcesses": [{"value": "Die Produktionsstufen sind Einwiegen, Mischen und Ausziehen der unvulkanisierten Rohlinge auf einem Kalander. Die anschließende Vulkanisation erfolgt kontinuierlich auf Fertigungslinien mit dampfbeheizten Trommel- oder Doppelbandpressen unter hohem Druck bei einer Temperatur von ca. 180°C zu 1,22 m breiten Bahnen. Nach der Vulkanisation werden die Bahnen rückseitig geschliffen und entweder als Rollenware aufgewickelt oder für Fliesenware abgelegt und gestanzt. Das Flächengewicht beträgt 5,08 kg/m². Das Qualitäts- und Energiemanagement der nora systems GmbH ist nach DIN EN ISO 9001 bzw. DIN EN ISO 50001 zertifiziert. \nTechnische Daten: \nAuszug aus technischen Datenblttern: (abrufbar auf www.nora.com) \nDeklarierte Einheit: \nAls Referenzgre wird 1 m Bodenbelag betrachtet. Die Werte des Moduls A1- A3 beziehen sich auf 1 m produziertes Produkt.\nEs handelt sich um eine Produktdeklaration. Die Herstellung und Beseitigung der Verschnitte bei der Installation werden dem Modul A5 zugeordnet. Die Module A1- A3, A4 und A5 beziehen sich gesamt auf 1 m installiertes Produkt.\nDie zur Installation notwendigen Materialien zur Vorbereitung des Untergrunds und zur Klebung werden nicht bercksichtigt. Fr den vollstndigen Bodenaufbau knnen Umweltproduktdeklarationen nach den IBU-PCR Dispersionsklebstoffe und –voranstriche sowie Mineralische Werkmrtel herangezogen werden.", "lang": "de"}, {"value": "The production stages are weighing, mixing, and stretching the unvulcanized blanks on a calender. The subsequent vulcanization takes place continuously on production lines with steam-heated drum or double belt presses under high pressure at a temperature of approx. 180°C to form 1.22 m wide webs. After vulcanization, the webs are ground on the back and either wound into rolls or cut into tiles and punched. The weight per unit area is 5.08 kg/m². The quality and energy management of nora systems GmbH is certified according to DIN EN ISO 9001 and DIN EN ISO 50001.\nTechnical data: \nExcerpt from technical data sheets: (available at www.nora.com) \nDeclared unit: \nThe reference unit is 1 m of floor covering. The values in modules A1-A3 refer to 1 m of manufactured product.\nThis is a product declaration. The production and disposal of offcuts during installation are assigned to module A5. Modules A1-A3, A4, and A5 refer to a total of 1 m of installed product.\nThe materials required for installation to prepare the substrate and for bonding are not taken into account. For the complete floor structure, environmental product declarations according to the IBU-PCR dispersion adhesives and primers as well as mineral mortars can be used.", "lang": "en"}], "technologicalApplicability": [{"value": "noraplan® 913 Bodenbelge sind fr verschiedene Anwendungsbereiche geeignet, zum Beispiel fr das Gesundheits- und Bildungswesen, die Industrie und Life Science, den ffentlichen Bau sowie fr die Verwendung in Shops und Stores. Fr die Verwendung und Anwendung gelten die jeweiligen nationalen Bestimmungen.\nDie Bodenbelge werden gem DIN EN ISO 10874 klassifiziert.", "lang": "de"}, {"value": "noraplan® 913 floor coverings are suitable for various application areas, such as for health and education, industry and life science, public building, and for use in shops and stores. The respective national regulations apply for use and application.\nThe floor coverings are classified according to DIN EN ISO 10874.", "lang": "en"}]}}, "modellingAndValidation": {"LCIMethodAndAllocation": {"typeOfDataSet": "EPD", "referenceToLCAMethodDetails": [{"shortDescription": [{"value": "Bodenbeläge.pdf", "lang": "de"}], "type": "source data set", "refObjectId": "a6d8257c-d16d-461d-811a-afba3911172b"}], "other": {"anies": [{"name": "subType", "value": "specific dataset"}]}}, "dataSourcesTreatmentAndRepresentativeness": {"referenceToDataSource": [{"shortDescription": [{"value": "GaBi Database (all versions)", "lang": "de"}], "type": "source data set", "refObjectId": "28d74cc0-db8b-4d7e-bc44-5f6d56ce0c4a"}, {"shortDescription": [{"value": "Sphera MLC (fka GaBi) CUP 2023.02", "lang": "de"}], "type": "source data set", "refObjectId": "cb600d3b-e85a-42b3-b059-5591e2757fbb"}], "useAdviceForDataSet": [{"value": "Gültigkeitsbereich: \nProduktfamilie noraplan® 913, mit einer Dicke von 3 mm. \nKontinuierlich in Bahnen vulkanisierte Bodenbelge aus Kautschuk in verschiedenen Farben und Designs. Diese Deklaration ist eine Umweltproduktdeklaration gem ISO 14025 und beschreibt die spezifische Umweltleistung der hier genannten Bauprodukte in Deutschland am Produktionsstandort Weinheim (Bergstrae). \nSystemgrenze: \nTyp der EPD: von der Wiege bis zum Werkstor mit Optionen.\nDie kobilanzielle Berechnung umfasst folgende\nPhasen:\nHerstellungsphase A1- A3: Bercksichtigung der Vorkette und der Produktion des\nBodenbelags, inkl. Verpackung (Input von Altpapier bei der Papier-/Kartonherstellung).\nTransport A4: Annahme fr den Transport der Produkte zur Baustelle.\nInstallationsphase A5: Bercksichtigung der Herstellung und des Transports der Verschnitt Menge, Verbrennung des Verschnitts (gewonnene Energie wird in D als vermiedene Umweltlasten deklariert), Entsorgung der Verpackungsmaterialien (Verbrennung der Polyethylenfolie). Die Untergrundvorbehandlung (Grundierung, Spachtelmasse, Klebstoff) bleibt unbercksichtigt. Diese ist abhngig vom Gebude und der Anwendung und muss im\nEinzelfall spezifiziert werden.\nNutzungsphase B2: Szenario fr die Reinigung entsprechend den Herstellerempfehlungen (siehe 4.).\nEnd-of-Life-Phase C1, C2, C3: Szenario fr die Verbrennung des Bodenbelags inkl.\nAusbau aus dem Gebude und Transport zum Verbrennungsort (gewonnene Energie\nwird in D als vermiedene Umweltlasten deklariert). Modul C4 wird mit 0 deklariert, da das EOL-Szenario keine Deponierung beinhaltet.\nNutzen und Lasten fr das nchste System D: Gewinnung von elektrischer und thermischer\nEnergie aus der thermischen Verwertung des Produkts, des Installationsverschnitts und der\nVerpackung Einflsse von Abfllen werden in den Modulen bercksichtigt, in denen diese anfallen.\nFr die Umweltauswirkungen wurde der Einsatz von grnem Strom unter Bercksichtigung des Reststrommixes fr den brigen Strom berechnet. Der Anteil des mit grnem Strom gedeckten Strombedarfs am Gesamtstrombedarf betrgt 100 %.", "lang": "de"}, {"value": "Scope of validity: \nProduct family noraplan® 913, with a thickness of 3 mm. \nContinuously vulcanized rubber floor coverings in various colors and designs. This declaration is an environmental product declaration according to ISO 14025 and describes the specific environmental performance of the construction products mentioned here in Germany at the production site in Weinheim (Bergstraße). \nSystem boundary: \nType of EPD: from cradle to gate with options.\nThe life cycle assessment calculation includes the following\nphases:\nManufacturing phase A1-A3: Consideration of the upstream chain and production of the\nfloor covering, including packaging (input of waste paper in paper/cardboard production).\nTransport A4: Assumption for the transport of products to the construction site.\nInstallation phase A5: Consideration of the production and transport of the cutting waste quantity, incineration of the cutting waste (recovered energy is declared in D as avoided environmental burdens), disposal of packaging materials (incineration of polyethylene film). The substrate pre-treatment (primer, filler, adhesive) is not considered. This depends on the building and application and must be\nspecified on a case-by-case basis.\nUse phase B2: Scenario for cleaning according to manufacturer recommendations (see 4.).\nEnd-of-life phase C1, C2, C3: Scenario for incineration of the floor covering including\nremoval from the building and transport to the incineration site (recovered energy\nis declared in D as avoided environmental burdens). Module C4 is declared as 0, as the EOL scenario does not include landfilling.\nBenefits and burdens for the next system D: Recovery of electrical and thermal\nenergy from the thermal recovery of the product, installation cutting waste and\npackaging. Waste influences are considered in the modules where they occur.\nFor environmental impacts, the use of green electricity was calculated taking into account the residual electricity mix for the remaining electricity. The share of electricity demand covered by green electricity of the total electricity demand is 100%.", "lang": "en"}], "other": {"anies": [{"name": "referenceToOriginalEPD", "value": {"shortDescription": {"value": "noraplan® 913 3 mm.pdf", "defaultValue": "noraplan® 913 3 mm.pdf", "lstrings": [{"lang": "de", "value": "noraplan® 913 3 mm.pdf"}]}, "type": "source data set", "uuid": {"uuid": "caad3a17-f94c-430b-8150-55c9373f7ea4"}, "refObjectId": "caad3a17-f94c-430b-8150-55c9373f7ea4", "resourceURLs": ["https://oekobaudat.de/OEKOBAU.DAT/resource/sources/caad3a17-f94c-430b-8150-55c9373f7ea4/noraplan_913_3_mm_20663.pdf?version=00.01.000"]}}]}}, "validation": {"review": [{"referenceToNameOfReviewerAndInstitution": [{"shortDescription": [{"value": "Institut Bauen und Umwelt e. V.", "lang": "de"}], "type": "contact data set", "refObjectId": "d111dbec-b024-4be5-86c5-752d6eb2cf95", "uri": "../contacts/d111dbec-b024-4be5-86c5-752d6eb2cf95.xml"}], "type": "Accredited third party review"}]}, "complianceDeclarations": {"compliance": [{"referenceToComplianceSystem": {"shortDescription": [{"value": "DIN EN 15804+A2", "lang": "de"}], "type": "source data set", "refObjectId": "c0016b33-8cf7-415c-ac6e-deba0d21440d", "uri": "../sources/c0016b33-8cf7-415c-ac6e-deba0d21440d.xml"}}, {"referenceToComplianceSystem": {"shortDescription": [{"value": "ISO 14025", "lang": "de"}], "type": "source data set", "refObjectId": "4f2eb655-6e44-4874-a95a-e28f5442cd4d", "uri": "../sources/4f2eb655-6e44-4874-a95a-e28f5442cd4d.xml"}}]}}, "administrativeInformation": {"commissionerAndGoal": {"referenceToCommissioner": [{"shortDescription": [{"value": "nora systems GmbH", "lang": "de"}], "type": "contact data set", "refObjectId": "6116f444-2f51-49a2-8f7e-82c2cbb7f3ff", "uri": "../contacts/6116f444-2f51-49a2-8f7e-82c2cbb7f3ff.xml"}]}, "dataGenerator": {"referenceToPersonOrEntityGeneratingTheDataSet": [{"shortDescription": [{"value": "Daxner & Merl GmbH", "lang": "de"}], "type": "contact data set", "refObjectId": "ad8ad627-3991-42b7-a7ca-5a3fe0a34c28", "uri": "../contacts/ad8ad627-3991-42b7-a7ca-5a3fe0a34c28.xml"}]}, "dataEntryBy": {"timeStamp": 1733356800000, "referenceToDataSetFormat": [{"shortDescription": [{"value": "ILCD Format", "lang": "de"}], "type": "source data set", "refObjectId": "a97a0155-0234-4b87-b4ce-a45da52f2a40", "uri": "../sources/a97a0155-0234-4b87-b4ce-a45da52f2a40.xml"}, {"shortDescription": [{"value": "EPD-Datenformaterweiterungen v1.2", "lang": "de"}, {"value": "EPD Data Format Extensions v1.2", "lang": "en"}], "type": "source data set", "refObjectId": "a29449fd-aa2f-4de8-b5d7-4b06b43c6fde", "uri": "../sources/a29449fd-aa2f-4de8-b5d7-4b06b43c6fde.xml"}]}, "publicationAndOwnership": {"dataSetVersion": "00.01.100", "referenceToPrecedingDataSetVersion": [{"shortDescription": [{"value": "noraplan® 913", "lang": "de"}], "type": "process data set", "refObjectId": "eec4acca-9f3c-4628-8298-9c53875034cf", "uri": "../processes/eec4acca-9f3c-4628-8298-9c53875034cf.xml"}], "referenceToRegistrationAuthority": {"shortDescription": [{"value": "Institut Bauen und Umwelt e. V.", "lang": "de"}], "type": "contact data set", "refObjectId": "d111dbec-b024-4be5-86c5-752d6eb2cf95", "uri": "../contacts/d111dbec-b024-4be5-86c5-752d6eb2cf95.xml"}, "registrationNumber": "EPD-NOR-20240466-IBA1-DE", "referenceToOwnershipOfDataSet": {"shortDescription": [{"value": "nora systems GmbH", "lang": "de"}], "type": "contact data set", "refObjectId": "6116f444-2f51-49a2-8f7e-82c2cbb7f3ff", "uri": "../contacts/6116f444-2f51-49a2-8f7e-82c2cbb7f3ff.xml"}, "copyright": true, "licenseType": "Free of charge for all users and uses", "accessRestrictions": [{"value": "None", "lang": "en"}], "other": {"anies": [{"name": "referenceToPublisher", "value": {"shortDescription": [{"value": "Institut Bauen und Umwelt e. V.", "lang": "de"}], "type": "contact data set", "refObjectId": "d111dbec-b024-4be5-86c5-752d6eb2cf95", "uri": "../contacts/d111dbec-b024-4be5-86c5-752d6eb2cf95.xml"}}]}}}, "exchanges": {"exchange": [{"dataSetInternalID": 0, "referenceToFlowDataSet": {"shortDescription": [{"value": "noraplan® 913/ 1 m2 (noraplan® 913/ 1 m2)", "lang": "de"}], "type": "flow data set", "refObjectId": "f76b95cf-4ede-c286-a5a9-d9e0dbea9887", "uri": "../flows/f76b95cf-4ede-c286-a5a9-d9e0dbea9887.xml"}, "meanAmount": 1.0, "referencesToDataSource": {}, "referenceFlow": true, "resolvedFlowVersion": "00.03.000", "resultingflowAmount": 1.0, "flowProperties": [{"name": [{"lang": "de", "value": "Fläche"}, {"lang": "en", "value": "Area"}], "uuid": "93a60a56-a3c8-19da-a746-0800200c9a66", "referenceFlowProperty": true, "meanValue": 1.0, "referenceUnit": "qm", "unitGroupUUID": "c20a03d7-bd90-4569-bc94-66cfd364dfc8"}], "materialProperties": [{"name": "gross density", "value": "3.36", "unit": "kg/m^3", "unitDescription": "kilograms per cubic metre"}, {"name": "grammage", "value": "3.36", "unit": "kg/m^2", "unitDescription": "kilograms per square meter"}, {"name": "layer thickness", "value": "0.002", "unit": "m", "unitDescription": "meters"}], "typeOfFlow": "Product flow", "classification": {"classHierarchy": "Kunststoffe / Bodenbeläge / Gummi-/Kautschuk-Bodenbeläge", "name": "OEKOBAU.DAT"}}, {"dataSetInternalID": 1, "referenceToFlowDataSet": {"shortDescription": [{"value": "Erneuerbare Primärenergie als Energieträger (PERE)", "lang": "de"}, {"value": "Renewable primary energy as energy carrier (PERE)", "lang": "en"}], "type": "flow data set", "refObjectId": "20f32be5-0398-4288-9b6d-accddd195317", "uri": "../flows/20f32be5-0398-4288-9b6d-accddd195317.xml"}, "exchange direction": "INPUT", "other": {"anies": [{"name": "referenceToUnitGroupDataSet", "value": {"shortDescription": [{"value": "MJ", "lang": "de"}], "type": "unit group data set", "refObjectId": "93a60a57-a3c8-11da-a746-0800200c9a66", "uri": "../unitgroups/93a60a57-a3c8-11da-a746-0800200c9a66.xml"}}, {"value": "20.8450394092215", "module": "A1-A3"}, {"value": "0.299288163569608", "module": "A4"}, {"value": "2.59095880286734", "module": "A5"}, {"value": "0.107034723276037", "module": "B2"}, {"value": "0.405820076487879", "module": "C1"}, {"value": "0.0148423529751138", "module": "C2"}, {"value": "25.900424191504", "module": "C3"}, {"value": "0", "module": "C4"}, {"value": "-6.89582870590441", "module": "D"}]}, "resolvedFlowVersion": "38.00.000", "flowProperties": [], "typeOfFlow": "Other flow", "classification": {"classHierarchy": "Quantities", "name": "GaBiCategories"}}, {"dataSetInternalID": 2, "referenceToFlowDataSet": {"shortDescription": [{"value": "Erneuerbare Primärenergie zur stofflichen Nutzung (PERM)", "lang": "de"}, {"value": "Renewable primary energy resources as material utilization (PERM)", "lang": "en"}], "type": "flow data set", "refObjectId": "fb3ec0de-548d-4508-aea5-00b73bf6f702", "uri": "../flows/fb3ec0de-548d-4508-aea5-00b73bf6f702.xml"}, "exchange direction": "INPUT", "other": {"anies": [{"name": "referenceToUnitGroupDataSet", "value": {"shortDescription": [{"value": "MJ", "lang": "de"}], "type": "unit group data set", "refObjectId": "93a60a57-a3c8-11da-a746-0800200c9a66", "uri": "../unitgroups/93a60a57-a3c8-11da-a746-0800200c9a66.xml"}}, {"value": "25.93594", "module": "A1-A3"}, {"value": "0", "module": "A4"}, {"value": "-0.1905", "module": "A5"}, {"value": "0", "module": "B2"}, {"value": "0", "module": "C1"}, {"value": "0", "module": "C2"}, {"value": "-25.74544", "module": "C3"}, {"value": "0", "module": "C4"}, {"value": "0", "module": "D"}]}, "resolvedFlowVersion": "38.00.000", "flowProperties": [], "typeOfFlow": "Other flow", "classification": {"classHierarchy": "Quantities", "name": "GaBiCategories"}}, {"dataSetInternalID": 3, "referenceToFlowDataSet": {"shortDescription": [{"value": "Total erneuerbare Primärenergie (PERT)", "lang": "de"}, {"value": "Total use of renewable primary energy resources (PERT)", "lang": "en"}], "type": "flow data set", "refObjectId": "53f97275-fa8a-4cdd-9024-65936002acd0", "uri": "../flows/53f97275-fa8a-4cdd-9024-65936002acd0.xml"}, "exchange direction": "INPUT", "other": {"anies": [{"name": "referenceToUnitGroupDataSet", "value": {"shortDescription": [{"value": "MJ", "lang": "de"}], "type": "unit group data set", "refObjectId": "93a60a57-a3c8-11da-a746-0800200c9a66", "uri": "../unitgroups/93a60a57-a3c8-11da-a746-0800200c9a66.xml"}}, {"value": "46.7809794092215", "module": "A1-A3"}, {"value": "0.299288163569608", "module": "A4"}, {"value": "2.40045880286734", "module": "A5"}, {"value": "0.107034723276037", "module": "B2"}, {"value": "0.405820076487879", "module": "C1"}, {"value": "0.0148423529751138", "module": "C2"}, {"value": "0.154984191503969", "module": "C3"}, {"value": "0", "module": "C4"}, {"value": "-6.89582870590441", "module": "D"}]}, "resolvedFlowVersion": "38.00.000", "flowProperties": [], "typeOfFlow": "Other flow", "classification": {"classHierarchy": "Quantities / Environmental quantities / EPD EN 15804 / LCI indicators", "name": "GaBiCategories"}}, {"dataSetInternalID": 4, "referenceToFlowDataSet": {"shortDescription": [{"value": "Nicht-erneuerbare Primärenergie als Energieträger (PENRE)", "lang": "de"}, {"value": "Non renewable primary energy as energy carrier (PENRE)", "lang": "en"}], "type": "flow data set", "refObjectId": "ac857178-2b45-46ec-892a-a9a4332f0372", "uri": "../flows/ac857178-2b45-46ec-892a-a9a4332f0372.xml"}, "exchange direction": "INPUT", "other": {"anies": [{"name": "referenceToUnitGroupDataSet", "value": {"shortDescription": [{"value": "MJ", "lang": "de"}], "type": "unit group data set", "refObjectId": "93a60a57-a3c8-11da-a746-0800200c9a66", "uri": "../unitgroups/93a60a57-a3c8-11da-a746-0800200c9a66.xml"}}, {"value": "128.201115772731", "module": "A1-A3"}, {"value": "4.64917668403745", "module": "A4"}, {"value": "8.73355805362295", "module": "A5"}, {"value": "2.32549438794639", "module": "B2"}, {"value": "0.679049388606871", "module": "C1"}, {"value": "0.204721342532753", "module": "C2"}, {"value": "37.1763446310741", "module": "C3"}, {"value": "0", "module": "C4"}, {"value": "-23.6157282897026", "module": "D"}]}, "resolvedFlowVersion": "38.00.000", "flowProperties": [], "typeOfFlow": "Other flow", "classification": {"classHierarchy": "Quantities", "name": "GaBiCategories"}}, {"dataSetInternalID": 5, "referenceToFlowDataSet": {"shortDescription": [{"value": "Nicht-erneuerbare Primärenergie zur stofflichen Nutzung (PENRM)", "lang": "de"}, {"value": "Non renewable primary energy as material utilization (PENRM)", "lang": "en"}], "type": "flow data set", "refObjectId": "1421caa0-679d-4bf4-b282-0eb850ccae27", "uri": "../flows/1421caa0-679d-4bf4-b282-0eb850ccae27.xml"}, "exchange direction": "INPUT", "other": {"anies": [{"name": "referenceToUnitGroupDataSet", "value": {"shortDescription": [{"value": "MJ", "lang": "de"}], "type": "unit group data set", "refObjectId": "93a60a57-a3c8-11da-a746-0800200c9a66", "uri": "../unitgroups/93a60a57-a3c8-11da-a746-0800200c9a66.xml"}}, {"value": "36.659428", "module": "A1-A3"}, {"value": "0", "module": "A4"}, {"value": "-0.088", "module": "A5"}, {"value": "0", "module": "B2"}, {"value": "0", "module": "C1"}, {"value": "0", "module": "C2"}, {"value": "-36.571428", "module": "C3"}, {"value": "0", "module": "C4"}, {"value": "0", "module": "D"}]}, "resolvedFlowVersion": "38.00.000", "flowProperties": [], "typeOfFlow": "Other flow", "classification": {"classHierarchy": "Quantities", "name": "GaBiCategories"}}, {"dataSetInternalID": 6, "referenceToFlowDataSet": {"shortDescription": [{"value": "Total nicht erneuerbare Primärenergie (PENRT)", "lang": "de"}, {"value": "Total use of non renewable primary energy resources (PENRT)", "lang": "en"}], "type": "flow data set", "refObjectId": "06159210-646b-4c8d-8583-da9b3b95a6c1", "uri": "../flows/06159210-646b-4c8d-8583-da9b3b95a6c1.xml"}, "exchange direction": "INPUT", "other": {"anies": [{"name": "referenceToUnitGroupDataSet", "value": {"shortDescription": [{"value": "MJ", "lang": "de"}], "type": "unit group data set", "refObjectId": "93a60a57-a3c8-11da-a746-0800200c9a66", "uri": "../unitgroups/93a60a57-a3c8-11da-a746-0800200c9a66.xml"}}, {"value": "164.860543772731", "module": "A1-A3"}, {"value": "4.64917668403745", "module": "A4"}, {"value": "8.64555805362295", "module": "A5"}, {"value": "2.32549438794639", "module": "B2"}, {"value": "0.679049388606871", "module": "C1"}, {"value": "0.204721342532753", "module": "C2"}, {"value": "0.604916631074108", "module": "C3"}, {"value": "0", "module": "C4"}, {"value": "-23.6157282897026", "module": "D"}]}, "resolvedFlowVersion": "38.00.000", "flowProperties": [], "typeOfFlow": "Other flow", "classification": {"classHierarchy": "Quantities / Environmental quantities / EPD EN 15804 / LCI indicators", "name": "GaBiCategories"}}, {"dataSetInternalID": 7, "referenceToFlowDataSet": {"shortDescription": [{"value": "Einsatz von Sekundärstoffen (SM)", "lang": "de"}, {"value": "Use of secondary material (SM)", "lang": "en"}], "type": "flow data set", "refObjectId": "c6a1f35f-2d09-4f54-8dfb-97e502e1ce92", "uri": "../flows/c6a1f35f-2d09-4f54-8dfb-97e502e1ce92.xml"}, "exchange direction": "INPUT", "other": {"anies": [{"name": "referenceToUnitGroupDataSet", "value": {"shortDescription": [{"value": "kg", "lang": "de"}], "type": "unit group data set", "refObjectId": "ad38d542-3fe9-439d-9b95-2f5f7752acaf", "uri": "../unitgroups/ad38d542-3fe9-439d-9b95-2f5f7752acaf.xml"}}, {"value": "0.039", "module": "A1-A3"}, {"value": "0", "module": "A4"}, {"value": "0", "module": "A5"}, {"value": "0", "module": "B2"}, {"value": "0", "module": "C1"}, {"value": "0", "module": "C2"}, {"value": "0", "module": "C3"}, {"value": "0", "module": "C4"}, {"value": "0", "module": "D"}]}, "resolvedFlowVersion": "38.00.000", "flowProperties": [], "typeOfFlow": "Other flow", "classification": {"classHierarchy": "Quantities / Environmental quantities / EPD EN 15804 / LCI indicators", "name": "GaBiCategories"}}, {"dataSetInternalID": 8, "referenceToFlowDataSet": {"shortDescription": [{"value": "Erneuerbare Sekundärbrennstoffe (RSF)", "lang": "de"}, {"value": "Use of renewable secondary fuels (RSF)", "lang": "en"}], "type": "flow data set", "refObjectId": "64333088-a55f-4aa2-9a31-c10b07816787", "uri": "../flows/64333088-a55f-4aa2-9a31-c10b07816787.xml"}, "exchange direction": "INPUT", "other": {"anies": [{"name": "referenceToUnitGroupDataSet", "value": {"shortDescription": [{"value": "MJ", "lang": "de"}], "type": "unit group data set", "refObjectId": "93a60a57-a3c8-11da-a746-0800200c9a66", "uri": "../unitgroups/93a60a57-a3c8-11da-a746-0800200c9a66.xml"}}, {"value": "0", "module": "A1-A3"}, {"value": "0", "module": "A4"}, {"value": "0", "module": "A5"}, {"value": "0", "module": "B2"}, {"value": "0", "module": "C1"}, {"value": "0", "module": "C2"}, {"value": "0", "module": "C3"}, {"value": "0", "module": "C4"}, {"value": "0", "module": "D"}]}, "resolvedFlowVersion": "38.00.000", "flowProperties": [], "typeOfFlow": "Other flow", "classification": {"classHierarchy": "Quantities / Environmental quantities / EPD EN 15804 / LCI indicators", "name": "GaBiCategories"}}, {"dataSetInternalID": 9, "referenceToFlowDataSet": {"shortDescription": [{"value": "Nicht erneuerbare Sekundärbrennstoffe (NRSF)", "lang": "de"}, {"value": "Use of non renewable secondary fuels (NRSF)", "lang": "en"}], "type": "flow data set", "refObjectId": "89def144-d39a-4287-b86f-efde453ddcb2", "uri": "../flows/89def144-d39a-4287-b86f-efde453ddcb2.xml"}, "exchange direction": "INPUT", "other": {"anies": [{"name": "referenceToUnitGroupDataSet", "value": {"shortDescription": [{"value": "MJ", "lang": "de"}], "type": "unit group data set", "refObjectId": "93a60a57-a3c8-11da-a746-0800200c9a66", "uri": "../unitgroups/93a60a57-a3c8-11da-a746-0800200c9a66.xml"}}, {"value": "0", "module": "A1-A3"}, {"value": "0", "module": "A4"}, {"value": "0", "module": "A5"}, {"value": "0", "module": "B2"}, {"value": "0", "module": "C1"}, {"value": "0", "module": "C2"}, {"value": "0", "module": "C3"}, {"value": "0", "module": "C4"}, {"value": "0", "module": "D"}]}, "resolvedFlowVersion": "38.00.000", "flowProperties": [], "typeOfFlow": "Other flow", "classification": {"classHierarchy": "Quantities / Environmental quantities / EPD EN 15804 / LCI indicators", "name": "GaBiCategories"}}, {"dataSetInternalID": 10, "referenceToFlowDataSet": {"shortDescription": [{"value": "Einsatz von Süßwasserressourcen (FW)", "lang": "de"}, {"value": "Use of net fresh water (FW)", "lang": "en"}], "type": "flow data set", "refObjectId": "3cf952c8-f3a4-461d-8c96-96456ca62246", "uri": "../flows/3cf952c8-f3a4-461d-8c96-96456ca62246.xml"}, "exchange direction": "INPUT", "other": {"anies": [{"name": "referenceToUnitGroupDataSet", "value": {"shortDescription": [{"value": "m^3", "lang": "de"}], "type": "unit group data set", "refObjectId": "cd950537-0a98-4044-9ba7-9f9a68d0a504", "uri": "../unitgroups/cd950537-0a98-4044-9ba7-9f9a68d0a504.xml"}}, {"value": "2.33071538890648", "module": "A1-A3"}, {"value": "0.000328343545918434", "module": "A4"}, {"value": "0.118847958371", "module": "A5"}, {"value": "0.00039246748669243", "module": "B2"}, {"value": "0.000327646301193307", "module": "C1"}, {"value": "1.62563767766023E-05", "module": "C2"}, {"value": "0.0075966518443883", "module": "C3"}, {"value": "0", "module": "C4"}, {"value": "-0.00558699237362512", "module": "D"}]}, "resolvedFlowVersion": "38.00.000", "flowProperties": [], "typeOfFlow": "Other flow", "classification": {"classHierarchy": "Quantities / Environmental quantities / EPD EN 15804 / LCI indicators", "name": "GaBiCategories"}}, {"dataSetInternalID": 11, "referenceToFlowDataSet": {"shortDescription": [{"value": "Gefährlicher Abfall zur Deponie (HWD)", "lang": "de"}, {"value": "Hazardous waste disposed (HWD)", "lang": "en"}], "type": "flow data set", "refObjectId": "430f9e0f-59b2-46a0-8e0d-55e0e84948fc", "uri": "../flows/430f9e0f-59b2-46a0-8e0d-55e0e84948fc.xml"}, "exchange direction": "OUTPUT", "other": {"anies": [{"name": "referenceToUnitGroupDataSet", "value": {"shortDescription": [{"value": "kg", "lang": "de"}], "type": "unit group data set", "refObjectId": "ad38d542-3fe9-439d-9b95-2f5f7752acaf", "uri": "../unitgroups/ad38d542-3fe9-439d-9b95-2f5f7752acaf.xml"}}, {"value": "1.31913056321736E-05", "module": "A1-A3"}, {"value": "1.44550407926027E-11", "module": "A4"}, {"value": "6.69995720324671E-07", "module": "A5"}, {"value": "0.000123702728485865", "module": "B2"}, {"value": "-5.31316657007104E-11", "module": "C1"}, {"value": "6.33882244946793E-13", "module": "C2"}, {"value": "1.07380824864536E-11", "module": "C3"}, {"value": "0", "module": "C4"}, {"value": "-1.24624765819277E-09", "module": "D"}]}, "resolvedFlowVersion": "38.00.000", "flowProperties": [], "typeOfFlow": "Other flow", "classification": {"classHierarchy": "Quantities / Environmental quantities / EPD EN 15804 / LCI indicators", "name": "GaBiCategories"}}, {"dataSetInternalID": 12, "referenceToFlowDataSet": {"shortDescription": [{"value": "Entsorgter nicht gefährlicher Abfall (NHWD)", "lang": "de"}, {"value": "Non hazardous waste disposed (NHWD)", "lang": "en"}], "type": "flow data set", "refObjectId": "b29ef66b-e286-4afa-949f-62f1a7b4d7fa", "uri": "../flows/b29ef66b-e286-4afa-949f-62f1a7b4d7fa.xml"}, "exchange direction": "OUTPUT", "other": {"anies": [{"name": "referenceToUnitGroupDataSet", "value": {"shortDescription": [{"value": "kg", "lang": "de"}], "type": "unit group data set", "refObjectId": "ad38d542-3fe9-439d-9b95-2f5f7752acaf", "uri": "../unitgroups/ad38d542-3fe9-439d-9b95-2f5f7752acaf.xml"}}, {"value": "3.57171897959391", "module": "A1-A3"}, {"value": "0.000674900605691797", "module": "A4"}, {"value": "0.187875222770355", "module": "A5"}, {"value": "0.00892204323308019", "module": "B2"}, {"value": "0.000497307497764054", "module": "C1"}, {"value": "3.12075470808382E-05", "module": "C2"}, {"value": "0.113445775819401", "module": "C3"}, {"value": "0", "module": "C4"}, {"value": "-0.0116808407613208", "module": "D"}]}, "resolvedFlowVersion": "38.00.000", "flowProperties": [], "typeOfFlow": "Other flow", "classification": {"classHierarchy": "Quantities / Environmental quantities / EPD EN 15804 / LCI indicators", "name": "GaBiCategories"}}, {"dataSetInternalID": 13, "referenceToFlowDataSet": {"shortDescription": [{"value": "Entsorgter radioaktiver Abfall (RWD)", "lang": "de"}, {"value": "Radioactive waste disposed (RWD)", "lang": "en"}], "type": "flow data set", "refObjectId": "3449546e-52ad-4b39-b809-9fb77cea8ff6", "uri": "../flows/3449546e-52ad-4b39-b809-9fb77cea8ff6.xml"}, "exchange direction": "OUTPUT", "other": {"anies": [{"name": "referenceToUnitGroupDataSet", "value": {"shortDescription": [{"value": "kg", "lang": "de"}], "type": "unit group data set", "refObjectId": "ad38d542-3fe9-439d-9b95-2f5f7752acaf", "uri": "../unitgroups/ad38d542-3fe9-439d-9b95-2f5f7752acaf.xml"}}, {"value": "0.00178468619209572", "module": "A1-A3"}, {"value": "8.31982578631707E-06", "module": "A4"}, {"value": "9.31032587350661E-05", "module": "A5"}, {"value": "4.89417927542667E-05", "module": "B2"}, {"value": "0.000107941069402033", "module": "C1"}, {"value": "3.83123816074733E-07", "module": "C2"}, {"value": "3.40894589428198E-05", "module": "C3"}, {"value": "0", "module": "C4"}, {"value": "-0.00182989485126353", "module": "D"}]}, "resolvedFlowVersion": "38.00.000", "flowProperties": [], "typeOfFlow": "Other flow", "classification": {"classHierarchy": "Quantities / Environmental quantities / EPD EN 15804 / LCI indicators", "name": "GaBiCategories"}}, {"dataSetInternalID": 14, "referenceToFlowDataSet": {"shortDescription": [{"value": "Komponenten für die Wiederverwendung (CRU)", "lang": "de"}, {"value": "Components for re-use (CRU)", "lang": "en"}], "type": "flow data set", "refObjectId": "a2b32f97-3fc7-4af2-b209-525bc6426f33", "uri": "../flows/a2b32f97-3fc7-4af2-b209-525bc6426f33.xml"}, "exchange direction": "OUTPUT", "other": {"anies": [{"name": "referenceToUnitGroupDataSet", "value": {"shortDescription": [{"value": "kg", "lang": "de"}], "type": "unit group data set", "refObjectId": "ad38d542-3fe9-439d-9b95-2f5f7752acaf", "uri": "../unitgroups/ad38d542-3fe9-439d-9b95-2f5f7752acaf.xml"}}, {"value": "0", "module": "A1-A3"}, {"value": "0", "module": "A4"}, {"value": "0", "module": "A5"}, {"value": "0", "module": "B2"}, {"value": "0", "module": "C1"}, {"value": "0", "module": "C2"}, {"value": "0", "module": "C3"}, {"value": "0", "module": "C4"}, {"value": "0", "module": "D"}]}, "resolvedFlowVersion": "38.00.000", "flowProperties": [], "typeOfFlow": "Other flow", "classification": {"classHierarchy": "Quantities / Environmental quantities / EPD EN 15804 / LCI indicators", "name": "GaBiCategories"}}, {"dataSetInternalID": 15, "referenceToFlowDataSet": {"shortDescription": [{"value": "Stoffe zum Recycling (MFR)", "lang": "de"}, {"value": "Materials for recycling (MFR)", "lang": "en"}], "type": "flow data set", "refObjectId": "d7fe48a5-4103-49c8-9aae-b0b5dfdbd6ae", "uri": "../flows/d7fe48a5-4103-49c8-9aae-b0b5dfdbd6ae.xml"}, "exchange direction": "OUTPUT", "other": {"anies": [{"name": "referenceToUnitGroupDataSet", "value": {"shortDescription": [{"value": "kg", "lang": "de"}], "type": "unit group data set", "refObjectId": "ad38d542-3fe9-439d-9b95-2f5f7752acaf", "uri": "../unitgroups/ad38d542-3fe9-439d-9b95-2f5f7752acaf.xml"}}, {"value": "0", "module": "A1-A3"}, {"value": "0", "module": "A4"}, {"value": "0", "module": "A5"}, {"value": "0", "module": "B2"}, {"value": "0", "module": "C1"}, {"value": "0", "module": "C2"}, {"value": "0", "module": "C3"}, {"value": "0", "module": "C4"}, {"value": "0", "module": "D"}]}, "resolvedFlowVersion": "38.00.000", "flowProperties": [], "typeOfFlow": "Other flow", "classification": {"classHierarchy": "Quantities / Environmental quantities / EPD EN 15804 / LCI indicators", "name": "GaBiCategories"}}, {"dataSetInternalID": 16, "referenceToFlowDataSet": {"shortDescription": [{"value": "Stoffe für die Energierückgewinnung (MER)", "lang": "de"}, {"value": "Materials for energy recovery (MER)", "lang": "en"}], "type": "flow data set", "refObjectId": "59a9181c-3aaf-46ee-8b13-2b3723b6e447", "uri": "../flows/59a9181c-3aaf-46ee-8b13-2b3723b6e447.xml"}, "exchange direction": "OUTPUT", "other": {"anies": [{"name": "referenceToUnitGroupDataSet", "value": {"shortDescription": [{"value": "kg", "lang": "de"}], "type": "unit group data set", "refObjectId": "ad38d542-3fe9-439d-9b95-2f5f7752acaf", "uri": "../unitgroups/ad38d542-3fe9-439d-9b95-2f5f7752acaf.xml"}}, {"value": "0", "module": "A1-A3"}, {"value": "0", "module": "A4"}, {"value": "0", "module": "A5"}, {"value": "0", "module": "B2"}, {"value": "0", "module": "C1"}, {"value": "0", "module": "C2"}, {"value": "0", "module": "C3"}, {"value": "0", "module": "C4"}, {"value": "0", "module": "D"}]}, "resolvedFlowVersion": "38.00.000", "flowProperties": [], "typeOfFlow": "Other flow", "classification": {"classHierarchy": "Quantities / Environmental quantities / EPD EN 15804 / LCI indicators", "name": "GaBiCategories"}}, {"dataSetInternalID": 17, "referenceToFlowDataSet": {"shortDescription": [{"value": "Exportierte elektrische Energie (EEE)", "lang": "de"}, {"value": "Exported electrical energy (EEE)", "lang": "en"}], "type": "flow data set", "refObjectId": "4da0c987-2b76-40d6-9e9e-82a017aaaf29", "uri": "../flows/4da0c987-2b76-40d6-9e9e-82a017aaaf29.xml"}, "exchange direction": "OUTPUT", "other": {"anies": [{"name": "referenceToUnitGroupDataSet", "value": {"shortDescription": [{"value": "MJ", "lang": "de"}], "type": "unit group data set", "refObjectId": "93a60a57-a3c8-11da-a746-0800200c9a66", "uri": "../unitgroups/93a60a57-a3c8-11da-a746-0800200c9a66.xml"}}, {"value": "0", "module": "A1-A3"}, {"value": "0", "module": "A4"}, {"value": "0.0247236078318369", "module": "A5"}, {"value": "0", "module": "B2"}, {"value": "0", "module": "C1"}, {"value": "0", "module": "C2"}, {"value": "5.74212505386232", "module": "C3"}, {"value": "0", "module": "C4"}, {"value": "0", "module": "D"}]}, "resolvedFlowVersion": "38.00.000", "flowProperties": [], "typeOfFlow": "Other flow", "classification": {"classHierarchy": "Quantities / Environmental quantities / EPD EN 15804 / LCI indicators", "name": "GaBiCategories"}}, {"dataSetInternalID": 18, "referenceToFlowDataSet": {"shortDescription": [{"value": "Exportierte thermische Energie (EET)", "lang": "de"}, {"value": "Exported thermal energy (EET)", "lang": "en"}], "type": "flow data set", "refObjectId": "98daf38a-7a79-46d3-9a37-2b7bd0955810", "uri": "../flows/98daf38a-7a79-46d3-9a37-2b7bd0955810.xml"}, "exchange direction": "OUTPUT", "other": {"anies": [{"name": "referenceToUnitGroupDataSet", "value": {"shortDescription": [{"value": "MJ", "lang": "de"}], "type": "unit group data set", "refObjectId": "93a60a57-a3c8-11da-a746-0800200c9a66", "uri": "../unitgroups/93a60a57-a3c8-11da-a746-0800200c9a66.xml"}}, {"value": "0", "module": "A1-A3"}, {"value": "0", "module": "A4"}, {"value": "0.0442190868133297", "module": "A5"}, {"value": "0", "module": "B2"}, {"value": "0", "module": "C1"}, {"value": "0", "module": "C2"}, {"value": "10.2859151801247", "module": "C3"}, {"value": "0", "module": "C4"}, {"value": "0", "module": "D"}]}, "resolvedFlowVersion": "38.00.000", "flowProperties": [], "typeOfFlow": "Other flow", "classification": {"classHierarchy": "Quantities / Environmental quantities / EPD EN 15804 / LCI indicators", "name": "GaBiCategories"}}]}, "LCIAResults": {"LCIAResult": [{"referenceToLCIAMethodDataSet": {"shortDescription": [{"value": "Globales Erwärmungspotenzial total (GWP-total)", "lang": "de"}, {"value": "Global Warming Potential total (GWP-total)", "lang": "en"}], "type": "LCIA method data set", "refObjectId": "6a37f984-a4b3-458a-a20a-64418c145fa2", "uri": "../lciamethods/6a37f984-a4b3-458a-a20a-64418c145fa2.xml"}, "other": {"anies": [{"name": "referenceToUnitGroupDataSet", "value": {"shortDescription": [{"value": "kg CO_(2)-Äq.", "lang": "de"}], "type": "unit group data set", "refObjectId": "1ebf3012-d0db-4de2-aefd-ef30cedb0be1", "uri": "../unitgroups/1ebf3012-d0db-4de2-aefd-ef30cedb0be1.xml"}}, {"value": "6.68775670138913", "module": "A1-A3"}, {"value": "0.345319671050297", "module": "A4"}, {"value": "0.57959537899093", "module": "A5"}, {"value": "0.0976656095666476", "module": "B2"}, {"value": "0.0325436184370899", "module": "C1"}, {"value": "0.0149605497168386", "module": "C2"}, {"value": "3.77544737446728", "module": "C3"}, {"value": "0", "module": "C4"}, {"value": "-1.28354050418874", "module": "D"}]}}, {"referenceToLCIAMethodDataSet": {"shortDescription": [{"value": "Globales Erwärmungspotenzial fossil (GWP-fossil)", "lang": "de"}, {"value": "Global Warming Potential fossil fuels (GWP-fossil)", "lang": "en"}], "type": "LCIA method data set", "refObjectId": "5f635281-343e-44fb-83df-1971b155e6b6", "uri": "../lciamethods/5f635281-343e-44fb-83df-1971b155e6b6.xml"}, "other": {"anies": [{"name": "referenceToUnitGroupDataSet", "value": {"shortDescription": [{"value": "kg CO_(2)-Äq.", "lang": "de"}], "type": "unit group data set", "refObjectId": "1ebf3012-d0db-4de2-aefd-ef30cedb0be1", "uri": "../unitgroups/1ebf3012-d0db-4de2-aefd-ef30cedb0be1.xml"}}, {"value": "8.40623923873084", "module": "A1-A3"}, {"value": "0.34182608092835", "module": "A4"}, {"value": "0.659148974898462", "module": "A5"}, {"value": "0.0929641241824758", "module": "B2"}, {"value": "0.0322596705162275", "module": "C1"}, {"value": "0.0147880310332376", "module": "C2"}, {"value": "1.59599692717406", "module": "C3"}, {"value": "0", "module": "C4"}, {"value": "-1.2775939199682", "module": "D"}]}}, {"referenceToLCIAMethodDataSet": {"shortDescription": [{"value": "Globales Erwärmungspotenzial biogen (GWP-biogenic)", "lang": "de"}, {"value": "Global Warming Potential biogenic (GWP-biogenic)", "lang": "en"}], "type": "LCIA method data set", "refObjectId": "2356e1ab-0185-4db5-86e5-16de51c7485c", "uri": "../lciamethods/2356e1ab-0185-4db5-86e5-16de51c7485c.xml"}, "other": {"anies": [{"name": "referenceToUnitGroupDataSet", "value": {"shortDescription": [{"value": "kg CO_(2)-Äq.", "lang": "de"}], "type": "unit group data set", "refObjectId": "1ebf3012-d0db-4de2-aefd-ef30cedb0be1", "uri": "../unitgroups/1ebf3012-d0db-4de2-aefd-ef30cedb0be1.xml"}}, {"value": "-2.53463047223483", "module": "A1-A3"}, {"value": "0.000719644007114439", "module": "A4"}, {"value": "-0.121148267436155", "module": "A5"}, {"value": "0.00469994715908199", "module": "B2"}, {"value": "0.000280441493056765", "module": "C1"}, {"value": "3.38606528239699E-05", "module": "C2"}, {"value": "2.17943047279774", "module": "C3"}, {"value": "0", "module": "C4"}, {"value": "-0.00586303360561724", "module": "D"}]}}, {"referenceToLCIAMethodDataSet": {"shortDescription": [{"value": "Globales Erwärmungspotenzial luluc (GWP-luluc)", "lang": "de"}, {"value": "Global Warming Potential luluc (GWP-luluc)", "lang": "en"}], "type": "LCIA method data set", "refObjectId": "4331bbdb-978a-490d-8707-eeb047f01a55", "uri": "../lciamethods/4331bbdb-978a-490d-8707-eeb047f01a55.xml"}, "other": {"anies": [{"name": "referenceToUnitGroupDataSet", "value": {"shortDescription": [{"value": "kg CO_(2)-Äq.", "lang": "de"}], "type": "unit group data set", "refObjectId": "1ebf3012-d0db-4de2-aefd-ef30cedb0be1", "uri": "../unitgroups/1ebf3012-d0db-4de2-aefd-ef30cedb0be1.xml"}}, {"value": "0.816147934893111", "module": "A1-A3"}, {"value": "0.00277394611483278", "module": "A4"}, {"value": "0.0415946715286224", "module": "A5"}, {"value": "1.5382250897199E-06", "module": "B2"}, {"value": "3.50642780562094E-06", "module": "C1"}, {"value": "0.000138658030777112", "module": "C2"}, {"value": "1.99744954811062E-05", "module": "C3"}, {"value": "0", "module": "C4"}, {"value": "-8.35506149339266E-05", "module": "D"}]}}, {"referenceToLCIAMethodDataSet": {"shortDescription": [{"value": "Abbau Potential der stratosphärischen Ozonschicht (ODP)", "lang": "de"}, {"value": "Depletion potential of the stratospheric ozone layer (ODP)", "lang": "en"}], "type": "LCIA method data set", "refObjectId": "b5c629d6-def3-11e6-bf01-fe55135034f3", "uri": "../lciamethods/b5c629d6-def3-11e6-bf01-fe55135034f3.xml"}, "other": {"anies": [{"name": "referenceToUnitGroupDataSet", "value": {"shortDescription": [{"value": "kg CFC11-Äq.", "lang": "de"}], "type": "unit group data set", "refObjectId": "d9e957c9-7309-4474-bf3a-7777df6c4e5b", "uri": "../unitgroups/d9e957c9-7309-4474-bf3a-7777df6c4e5b.xml"}}, {"value": "2.21000656636562E-08", "module": "A1-A3"}, {"value": "4.20889940424809E-14", "module": "A4"}, {"value": "1.12249232119827E-09", "module": "A5"}, {"value": "8.11099503472155E-12", "module": "B2"}, {"value": "5.95266988800881E-13", "module": "C1"}, {"value": "1.9480525255647E-15", "module": "C2"}, {"value": "2.45020638597436E-13", "module": "C3"}, {"value": "0", "module": "C4"}, {"value": "-1.00995920783823E-11", "module": "D"}]}}, {"referenceToLCIAMethodDataSet": {"shortDescription": [{"value": "Versauerungspotenzial von Boden und Wasser (AP)", "lang": "de"}, {"value": "Acidification potential of land and water (AP)", "lang": "en"}], "type": "LCIA method data set", "refObjectId": "b5c611c6-def3-11e6-bf01-fe55135034f3", "uri": "../lciamethods/b5c611c6-def3-11e6-bf01-fe55135034f3.xml"}, "other": {"anies": [{"name": "referenceToUnitGroupDataSet", "value": {"shortDescription": [{"value": "mol H^(+)-Äq.", "lang": "de"}], "type": "unit group data set", "refObjectId": "42e089ac-92bf-4bf2-8ca1-5fc40d18f2ed", "uri": "../unitgroups/42e089ac-92bf-4bf2-8ca1-5fc40d18f2ed.xml"}}, {"value": "0.0561990111376399", "module": "A1-A3"}, {"value": "0.00258361488641578", "module": "A4"}, {"value": "0.00300758824566367", "module": "A5"}, {"value": "0.000294054388581696", "module": "B2"}, {"value": "6.89000731500695E-05", "module": "C1"}, {"value": "4.83086846069717E-05", "module": "C2"}, {"value": "0.000364180571704823", "module": "C3"}, {"value": "0", "module": "C4"}, {"value": "-0.00160326770127287", "module": "D"}]}}, {"referenceToLCIAMethodDataSet": {"shortDescription": [{"value": "Eutrophierungspotenzial Süßwasser (EP-freshwater)", "lang": "de"}, {"value": "Eutrophication potential aquatic freshwater (EP-freshwater)", "lang": "en"}], "type": "LCIA method data set", "refObjectId": "b53ec18f-7377-4ad3-86eb-cc3f4f276b2b", "uri": "../lciamethods/b53ec18f-7377-4ad3-86eb-cc3f4f276b2b.xml"}, "other": {"anies": [{"name": "referenceToUnitGroupDataSet", "value": {"shortDescription": [{"value": "kg P-Äq.", "lang": "de"}], "type": "unit group data set", "refObjectId": "0429039d-a61d-4590-ba67-aa4a20a810a1", "uri": "../unitgroups/0429039d-a61d-4590-ba67-aa4a20a810a1.xml"}}, {"value": "0.0010460804433168", "module": "A1-A3"}, {"value": "1.10519263887289E-06", "module": "A4"}, {"value": "5.31932406105427E-05", "module": "A5"}, {"value": "5.60741658871437E-06", "module": "B2"}, {"value": "1.20349557723587E-07", "module": "C1"}, {"value": "5.4737587300048E-08", "module": "C2"}, {"value": "1.04567082647397E-07", "module": "C3"}, {"value": "0", "module": "C4"}, {"value": "-2.08312576159307E-06", "module": "D"}]}}, {"referenceToLCIAMethodDataSet": {"shortDescription": [{"value": "Eutrophierungspotenzial Salzwasser (EP-marine)", "lang": "de"}, {"value": "Eutrophication potential aquatic marine (EP-marine)", "lang": "en"}], "type": "LCIA method data set", "refObjectId": "b5c619fa-def3-11e6-bf01-fe55135034f3", "uri": "../lciamethods/b5c619fa-def3-11e6-bf01-fe55135034f3.xml"}, "other": {"anies": [{"name": "referenceToUnitGroupDataSet", "value": {"shortDescription": [{"value": "kg N-Äq.", "lang": "de"}], "type": "unit group data set", "refObjectId": "d05bb823-ecdf-4686-8c40-bf1d9257859f", "uri": "../unitgroups/d05bb823-ecdf-4686-8c40-bf1d9257859f.xml"}}, {"value": "0.0104829189406403", "module": "A1-A3"}, {"value": "0.000817835235958172", "module": "A4"}, {"value": "0.000579703583721061", "module": "A5"}, {"value": "7.2297124390965E-05", "module": "B2"}, {"value": "1.648473098396E-05", "module": "C1"}, {"value": "2.18844928021642E-05", "module": "C2"}, {"value": "9.49444943024039E-05", "module": "C3"}, {"value": "0", "module": "C4"}, {"value": "-0.000468244060663161", "module": "D"}]}}, {"referenceToLCIAMethodDataSet": {"shortDescription": [{"value": "Eutrophierungspotenzial Land (EP-terrestrial)", "lang": "de"}, {"value": "Eutrophication potential terrestrial (EP-terrestrial)", "lang": "en"}], "type": "LCIA method data set", "refObjectId": "b5c614d2-def3-11e6-bf01-fe55135034f3", "uri": "../lciamethods/b5c614d2-def3-11e6-bf01-fe55135034f3.xml"}, "other": {"anies": [{"name": "referenceToUnitGroupDataSet", "value": {"shortDescription": [{"value": "mol N-Äq.", "lang": "de"}], "type": "unit group data set", "refObjectId": "71b4d617-0ec9-4d3f-b65e-e438940c2401", "uri": "../unitgroups/71b4d617-0ec9-4d3f-b65e-e438940c2401.xml"}}, {"value": "0.141803523655998", "module": "A1-A3"}, {"value": "0.00908493918022532", "module": "A4"}, {"value": "0.00776673989368069", "module": "A5"}, {"value": "0.000558631167170453", "module": "B2"}, {"value": "0.000172247725539726", "module": "C1"}, {"value": "0.000246081634066701", "module": "C2"}, {"value": "0.00171878140370203", "module": "C3"}, {"value": "0", "module": "C4"}, {"value": "-0.00501260485139835", "module": "D"}]}}, {"referenceToLCIAMethodDataSet": {"shortDescription": [{"value": "Bildungspotential für troposphärisches Ozon (POCP)", "lang": "de"}, {"value": "Formation potential of tropospheric ozone photochemical oxidants (POCP)", "lang": "en"}], "type": "LCIA method data set", "refObjectId": "b5c610fe-def3-11e6-bf01-fe55135034f3", "uri": "../lciamethods/b5c610fe-def3-11e6-bf01-fe55135034f3.xml"}, "other": {"anies": [{"name": "referenceToUnitGroupDataSet", "value": {"shortDescription": [{"value": "kg NMVOC-Äq.", "lang": "de"}], "type": "unit group data set", "refObjectId": "d27c25f8-fbc1-44c6-b47b-4adbae4199c6", "uri": "../unitgroups/d27c25f8-fbc1-44c6-b47b-4adbae4199c6.xml"}}, {"value": "0.0308619112199414", "module": "A1-A3"}, {"value": "0.00195648711913637", "module": "A4"}, {"value": "0.00168315713797586", "module": "A5"}, {"value": "0.000294874250555615", "module": "B2"}, {"value": "4.39784262164529E-05", "module": "C1"}, {"value": "4.36799591172108E-05", "module": "C2"}, {"value": "0.000270177927174758", "module": "C3"}, {"value": "0", "module": "C4"}, {"value": "-0.0013042310371391", "module": "D"}]}}, {"referenceToLCIAMethodDataSet": {"shortDescription": [{"value": "Potenzial für den abiotischen Abbau nicht fossiler Ressourcen (ADPE)", "lang": "de"}, {"value": "Abiotic depletion potential for non fossil resources (ADPE)", "lang": "en"}], "type": "LCIA method data set", "refObjectId": "b2ad6494-c78d-11e6-9d9d-cec0c932ce01", "uri": "../lciamethods/b2ad6494-c78d-11e6-9d9d-cec0c932ce01.xml"}, "other": {"anies": [{"name": "referenceToUnitGroupDataSet", "value": {"shortDescription": [{"value": "kg Sb-Äq.", "lang": "de"}], "type": "unit group data set", "refObjectId": "54ccd2d9-a32a-4fc2-923d-f2c8c93e89d4", "uri": "../unitgroups/54ccd2d9-a32a-4fc2-923d-f2c8c93e89d4.xml"}}, {"value": "0.000217923137094204", "module": "A1-A3"}, {"value": "2.02670250503173E-08", "module": "A4"}, {"value": "1.10696173116878E-05", "module": "A5"}, {"value": "1.64854570208129E-08", "module": "B2"}, {"value": "4.98945007650019E-09", "module": "C1"}, {"value": "9.9262183967809E-10", "module": "C2"}, {"value": "2.3752425880605E-09", "module": "C3"}, {"value": "0", "module": "C4"}, {"value": "-9.22241517496168E-08", "module": "D"}]}}, {"referenceToLCIAMethodDataSet": {"shortDescription": [{"value": "Potenzial für den abiotischen Abbau fossiler Brennstoffe (ADPF)", "lang": "de"}, {"value": "Abiotic depletion potential for fossil resources (ADPF)", "lang": "en"}], "type": "LCIA method data set", "refObjectId": "b2ad6110-c78d-11e6-9d9d-cec0c932ce01", "uri": "../lciamethods/b2ad6110-c78d-11e6-9d9d-cec0c932ce01.xml"}, "other": {"anies": [{"name": "referenceToUnitGroupDataSet", "value": {"shortDescription": [{"value": "MJ", "lang": "de"}], "type": "unit group data set", "refObjectId": "93a60a57-a3c8-11da-a746-0800200c9a66", "uri": "../unitgroups/93a60a57-a3c8-11da-a746-0800200c9a66.xml"}}, {"value": "164.714104267561", "module": "A1-A3"}, {"value": "4.63233891064091", "module": "A4"}, {"value": "8.63723382318891", "module": "A5"}, {"value": "2.32540338417642", "module": "B2"}, {"value": "0.678887523500628", "module": "C1"}, {"value": "0.203949734907582", "module": "C2"}, {"value": "0.604390023684261", "module": "C3"}, {"value": "0", "module": "C4"}, {"value": "-23.6126032369665", "module": "D"}]}}, {"referenceToLCIAMethodDataSet": {"shortDescription": [{"value": "Wassernutzung (WDP)", "lang": "de"}, {"value": "Water use (WDP)", "lang": "en"}], "type": "LCIA method data set", "refObjectId": "b2ad66ce-c78d-11e6-9d9d-cec0c932ce01", "uri": "../lciamethods/b2ad66ce-c78d-11e6-9d9d-cec0c932ce01.xml"}, "other": {"anies": [{"name": "referenceToUnitGroupDataSet", "value": {"shortDescription": [{"value": "m^(3) Welt-Äq. entzogen", "lang": "de"}], "type": "unit group data set", "refObjectId": "6ae2df01-888e-46c8-b17d-49fa3869b476", "uri": "../unitgroups/6ae2df01-888e-46c8-b17d-49fa3869b476.xml"}}, {"value": "19.7407462876402", "module": "A1-A3"}, {"value": "0.00369440708521823", "module": "A4"}, {"value": "1.02211664452413", "module": "A5"}, {"value": "0.0159794102491602", "module": "B2"}, {"value": "0.00718907633720711", "module": "C1"}, {"value": "0.000180912474603967", "module": "C2"}, {"value": "0.323504357625699", "module": "C3"}, {"value": "0", "module": "C4"}, {"value": "-0.122360355938737", "module": "D"}]}}, {"referenceToLCIAMethodDataSet": {"shortDescription": [{"value": "Auftreten von Krankheiten aufgrund von Feinstaubemissionen (PM)", "lang": "de"}, {"value": "Incidence of disease due to PM emissions (PM)", "lang": "en"}], "type": "LCIA method data set", "refObjectId": "b5c602c6-def3-11e6-bf01-fe55135034f3", "uri": "../lciamethods/b5c602c6-def3-11e6-bf01-fe55135034f3.xml"}, "other": {"anies": [{"name": "referenceToUnitGroupDataSet", "value": {"shortDescription": [{"value": "Krankheitsfälle", "lang": "de"}], "type": "unit group data set", "refObjectId": "3883559b-648f-4afc-8ba2-0bd24f3affa3", "uri": "../unitgroups/3883559b-648f-4afc-8ba2-0bd24f3affa3.xml"}}, {"value": "6.84493633437395E-07", "module": "A1-A3"}, {"value": "3.41082717227939E-08", "module": "A4"}, {"value": "3.67012351370448E-08", "module": "A5"}, {"value": "3.80559870411732E-09", "module": "B2"}, {"value": "5.79960438353899E-10", "module": "C1"}, {"value": "2.98122211212155E-10", "module": "C2"}, {"value": "3.46033787187624E-09", "module": "C3"}, {"value": "0", "module": "C4"}, {"value": "-1.36029021510334E-08", "module": "D"}]}}, {"referenceToLCIAMethodDataSet": {"shortDescription": [{"value": "Wirkung durch Exposition des Menschen mit U235 (IR)", "lang": "de"}, {"value": "Human exposure efficiency relative to U235 (IR)", "lang": "en"}], "type": "LCIA method data set", "refObjectId": "b5c632be-def3-11e6-bf01-fe55135034f3", "uri": "../lciamethods/b5c632be-def3-11e6-bf01-fe55135034f3.xml"}, "other": {"anies": [{"name": "referenceToUnitGroupDataSet", "value": {"shortDescription": [{"value": "kBq U235-Äq.", "lang": "de"}], "type": "unit group data set", "refObjectId": "456b05bf-1415-44a9-9993-02452f554c09", "uri": "../unitgroups/456b05bf-1415-44a9-9993-02452f554c09.xml"}}, {"value": "0.217871350510836", "module": "A1-A3"}, {"value": "0.00123684068228241", "module": "A4"}, {"value": "0.0114525810574738", "module": "A5"}, {"value": "0.0369355906244859", "module": "B2"}, {"value": "0.0179630403745954", "module": "C1"}, {"value": "5.71337189417765E-05", "module": "C2"}, {"value": "0.00542187979430191", "module": "C3"}, {"value": "0", "module": "C4"}, {"value": "-0.304393965574219", "module": "D"}]}}, {"referenceToLCIAMethodDataSet": {"shortDescription": [{"value": "Toxizitätsvergleichseinheit für Ökosysteme (ETP-fw)", "lang": "de"}, {"value": "Comparative toxic unit for ecosystems (ETP-fw)", "lang": "en"}], "type": "LCIA method data set", "refObjectId": "ee1082d1-b0f7-43ca-a1f0-21e2a4a74511", "uri": "../lciamethods/ee1082d1-b0f7-43ca-a1f0-21e2a4a74511.xml"}, "other": {"anies": [{"name": "referenceToUnitGroupDataSet", "value": {"shortDescription": [{"value": "CTUe", "lang": "de"}], "type": "unit group data set", "refObjectId": "aa959ded-f1eb-4efb-9c5c-2d60be36b3e6", "uri": "../unitgroups/aa959ded-f1eb-4efb-9c5c-2d60be36b3e6.xml"}}, {"value": "125.987733445764", "module": "A1-A3"}, {"value": "3.31266245240618", "module": "A4"}, {"value": "6.58409221490369", "module": "A5"}, {"value": "0.520835653712767", "module": "B2"}, {"value": "0.188655083238538", "module": "C1"}, {"value": "0.146092086190317", "module": "C2"}, {"value": "0.285667120722207", "module": "C3"}, {"value": "0", "module": "C4"}, {"value": "-3.30307598830273", "module": "D"}]}}, {"referenceToLCIAMethodDataSet": {"shortDescription": [{"value": "Toxizitätsvergleichseinheit für Menschen (krebserregend) (HTP-c)", "lang": "de"}, {"value": "Comparative toxic unit for humans (carcinogenic) (HTP-c)", "lang": "en"}], "type": "LCIA method data set", "refObjectId": "2299222a-bbd8-474f-9d4f-4dd1f18aea7c", "uri": "../lciamethods/2299222a-bbd8-474f-9d4f-4dd1f18aea7c.xml"}, "other": {"anies": [{"name": "referenceToUnitGroupDataSet", "value": {"shortDescription": [{"value": "CTUh", "lang": "de"}], "type": "unit group data set", "refObjectId": "d4c9523e-2d7e-49fd-8469-998f547d3a70", "uri": "../unitgroups/d4c9523e-2d7e-49fd-8469-998f547d3a70.xml"}}, {"value": "4.90325461890192E-09", "module": "A1-A3"}, {"value": "6.64159179193832E-11", "module": "A4"}, {"value": "2.53827854042819E-10", "module": "A5"}, {"value": "3.65552029846391E-11", "module": "B2"}, {"value": "9.98921128570414E-12", "module": "C1"}, {"value": "2.96438673845856E-12", "module": "C2"}, {"value": "2.34150727607166E-11", "module": "C3"}, {"value": "0", "module": "C4"}, {"value": "-2.61741005037546E-10", "module": "D"}]}}, {"referenceToLCIAMethodDataSet": {"shortDescription": [{"value": "Toxizitätsvergleichseinheit für Menschen (nicht krebserregend) (HTP-nc)", "lang": "de"}, {"value": "Comparative toxic unit for humans (noncarcinogenic) (HTP-nc)", "lang": "en"}], "type": "LCIA method data set", "refObjectId": "3af763a5-b7a1-48c9-9cee-1f223481fcef", "uri": "../lciamethods/3af763a5-b7a1-48c9-9cee-1f223481fcef.xml"}, "other": {"anies": [{"name": "referenceToUnitGroupDataSet", "value": {"shortDescription": [{"value": "CTUh", "lang": "de"}], "type": "unit group data set", "refObjectId": "d4c9523e-2d7e-49fd-8469-998f547d3a70", "uri": "../unitgroups/d4c9523e-2d7e-49fd-8469-998f547d3a70.xml"}}, {"value": "2.87120492348782E-07", "module": "A1-A3"}, {"value": "2.86554547353245E-09", "module": "A4"}, {"value": "1.475679057095E-08", "module": "A5"}, {"value": "3.04259945196637E-09", "module": "B2"}, {"value": "1.59236384350205E-10", "module": "C1"}, {"value": "1.31889029820805E-10", "module": "C2"}, {"value": "4.24551241023006E-10", "module": "C3"}, {"value": "0", "module": "C4"}, {"value": "-6.42660506173847E-09", "module": "D"}]}}, {"referenceToLCIAMethodDataSet": {"shortDescription": [{"value": "Bodenqualitätsindex (SQP)", "lang": "de"}, {"value": "Soil quality index (SQP)", "lang": "en"}], "type": "LCIA method data set", "refObjectId": "b2ad6890-c78d-11e6-9d9d-cec0c932ce01", "uri": "../lciamethods/b2ad6890-c78d-11e6-9d9d-cec0c932ce01.xml"}, "other": {"anies": [{"name": "referenceToUnitGroupDataSet", "value": {"shortDescription": [{"value": "SQP", "lang": "de"}], "type": "unit group data set", "refObjectId": "f130951c-e67f-4f7f-8dd4-665de3974e18", "uri": "../unitgroups/f130951c-e67f-4f7f-8dd4-665de3974e18.xml"}}, {"value": "768.019703270239", "module": "A1-A3"}, {"value": "1.70620479995163", "module": "A4"}, {"value": "39.1062836531524", "module": "A5"}, {"value": "0.0350532551272193", "module": "B2"}, {"value": "0.266424721171552", "module": "C1"}, {"value": "0.0852184104775424", "module": "C2"}, {"value": "0.192447449501941", "module": "C3"}, {"value": "0", "module": "C4"}, {"value": "-4.53424323673611", "module": "D"}]}}]}, "otherAttributes": {"{http://www.indata.network/EPD/2019}epd-version": "1.2"}, "version": "1.1", "locations": "../ILCDLocations.xml"}