{"processInformation": {"dataSetInformation": {"UUID": "7290c768-0a2c-4503-bd81-a7c27edc4541", "name": {"baseName": [{"value": "Kalzip® – Stehfalzsystem für Dachdeckungen und Wandbekleidungen aus Aluminium", "lang": "de"}, {"value": "Aluminium Standing Seam Roofing and Wall Cladding System - Kalzip®", "lang": "en"}], "functionalUnitFlowProperties": [{"lang": "de"}]}, "classificationInformation": {"classification": [{"class": [{"value": "Metalle", "level": 0, "classId": "4"}, {"value": "Aluminium", "level": 1, "classId": "4.3"}, {"value": "Aluminiumprofil", "level": 2, "classId": "4.3.02"}], "name": "OEKOBAU.DAT"}, {"class": [{"value": "02 Bauprodukte", "level": 0}, {"value": "Bedachungen", "level": 1}, {"value": "Bedachungs- und Fassadensysteme aus Aluminium", "level": 2}], "name": "IBUCategories"}]}, "generalComment": [{"value": "Das Stehfalzsystem aus Aluminium ist ein Dach- und Wandsystem aus profiliertem Dnnblech, das entweder werkseitig oder durch mobiles Rollformen am Projektort hergestellt werden kann. Es sind mehrere Profiltafelbreiten und -hhen verfgbar, um die verschiedenen Entwurfs-spezifikationen und Anforderungen an die Tragfhigkeit zu erfllen. Des Weiteren stehen verschiedene Material-oberflchen und Oberflchenbehandlungen zur Auswahl. Die Profiltafeln knnen in gerader, konvex- oder konkav-gerundeter, Freiform, konischer oder konisch-gerundeter Form sowie in Kombinationen aus Vorgenanntem geliefert werden.\nDas beschriebene System (Aluminiumblech mit PVDF-beschichteter Oberflche) stellt das System mit den hchsten Umweltwirkungen dar, um die Spanne der mglichen Varianten, die Kalzip fertigt, mit dieser EPD ebenfalls abzudecken.", "lang": "de"}, {"value": "The aluminium standing seam system is a roofing and wall cladding system made of profiled thin sheet metal that can be fabricated either in the factory or by mobile roll forming at the project site. Several profiled sheet panel widths and heights are available to meet different design specifications and load bearing requirements. Furthermore, various material finishes and surface treatments are available. The panels can be supplied in straight, convex- or concave-rounded, free-form, conical or conical-rounded shapes as well as in combinations of the above. The system described (aluminium sheet with PVDF-coated surface) represents the system with the highest environmental impact in order to also cover the range of possible variants that Kalzip manufactures with this EPD.", "lang": "en"}]}, "quantitativeReference": {"referenceToReferenceFlow": [0]}, "time": {"referenceYear": 2023, "dataSetValidUntil": 2028, "other": {"anies": [{"name": "publicationDateOfEPD", "value": 1681257600000}]}}, "geography": {"locationOfOperationSupplyOrProduction": {"location": "DE"}}, "technology": {"technologyDescriptionAndIncludedProcesses": [{"value": "Das Profilieren der Aluminiumbleche erfolgt firmenintern in der Produktionsstätte in Deutschland (elektronisch gesteuertes Verfahren). Beim Profilieren je 1m² werden 0,122 MJ Strom und 0,015 kg Schmiermittel verbraucht. Die stehende Stehfalzprofiltafel ist galvanisch veredelt (Zink). Die Dämm- und weitere Baustoffe werden extern zugekauft und auf der Baustelle zusammengebaut. \nDeklarierte Einheit: \nDiese EPD bezieht sich auf 1 m Stehfalzsystem fr Dachdeckungen und Wandbekleidungen aus Aluminium inkl. Verpackung.", "lang": "de"}, {"value": "The aluminium sheets are profiled in-house at the production facility in Germany (electronically controlled process). Profiling 1m² consumes 0.122 MJ of electricity and 0.015 kg of lubricant. The standing seam profile panel is finished with PVDF. The insulation and other building materials are purchased externally and assembled on site. \nDeclared unit: \nThis EPD refers to 1 m aluminium standing seam roofing and wall cladding system incl. packaging.", "lang": "en"}], "technologicalApplicability": [{"value": "Die Dachprofiltafeln aus Aluminium sind Profiltafeln, die durch mechanische Verbrdelung der seitlichen Randrippen benachbarter Dachelemente zu einem Stehfalz aneinandergefgt und als Auenhlle fr Dachdeckungen und Wandbekleidungen verwendet werden. Die Profiltafeln sind als Warm- und Kaltdachausfhrung fr alle Dachformen und Dachneigungen ab 1,5 Grad sowie fr alle Unterkonstruktionen und Tragwerke geeignet. Sie knnen sowohl bei Neubau- als auch bei Sanierungsvorhaben eingesetzt werden. Der konstruktive Aufbau richtet sich nach dem jeweiligen Anwendungsfall und lsst sich durch Wahl der geeigneten Dmmdicke exakt auf die erforderlichen U-Werte und Schall-dmmwerte des Gebudes anpassen. Industriell gefertigte Profiltafeln kommen in einer Vielzahl von Anwendungs-bereichen des Bauwesens zum Einsatz. Typische Anwendungsbeispiele sind Gebudehllen und Innenverkleidungen.", "lang": "de"}, {"value": "The aluminium profiled roof panels are profiled panels that are joined together by mechanically flanging the lateral edge ribs of adjacent roof elements to form a standing seam and are used as an outer shell for roofing and wall cladding. The profiled panels are suitable as warm and cold roof versions for all roof shapes and roof pitches from 1.5 degrees and for all substructures and supporting structures. They can be used for both new construction and renovation projects. The structural design depends on the respective application and can be adapted exactly to the required U-values and sound insulation values of the building by selecting the appropriate insulation thickness. Industrially manufactured profiled panels are used in a wide range of applications in the building industry. Typical applications include building envelopes and interior cladding.", "lang": "en"}]}}, "modellingAndValidation": {"LCIMethodAndAllocation": {"typeOfDataSet": "EPD", "referenceToLCAMethodDetails": [{"shortDescription": [{"value": "Bedachungs- und Fassadensysteme aus Aluminium.pdf", "lang": "de"}], "type": "source data set", "refObjectId": "bae56ae2-2177-48aa-a821-8f27001f3841"}], "other": {"anies": [{"name": "subType", "value": "representative dataset"}]}}, "dataSourcesTreatmentAndRepresentativeness": {"referenceToDataSource": [{"shortDescription": [{"value": "GaBi Database (all versions)", "lang": "de"}], "type": "source data set", "refObjectId": "28d74cc0-db8b-4d7e-bc44-5f6d56ce0c4a"}, {"shortDescription": [{"value": "GaBi Database Edition 2022, CUP 2022.02", "lang": "de"}], "type": "source data set", "refObjectId": "94f442cb-662e-43ea-a792-4b0a35132e93"}], "useAdviceForDataSet": [{"value": "Gültigkeitsbereich: \nDie vorliegende EPD bezieht sich auf Herstellung, Transport, Installation und Entsorgung von einem reprsentativen Produkt mit den hchsten Umweltwirkungen (Worst-Case) fr eine Spanne von Produkten (Stehfalzsystem fr Dachdeckungen und Wandbekleidungen) von Kalzip. Die technischen Eigenschaften werden in Kapitel 2.3 dargestellt. Produktionsstandort des Produkts ist Koblenz, Deutschland, von wo aus die Produkte direkt auf die kundenseitigen Baustellen ausgeliefert werden. \nSystemgrenze: \nTyp der EPD: Wiege bis Werkstor – mit Optionen (Modul A1–A3, A5, C1–4 und D).\n\nModule A1–A3\nDas Produktstadium enthlt die Produktion der notwendigen Rohstoffe inklusive aller Vorketten sowie der notwendigen Beschaffungstransporte. Fr die Produktion der deklarierten Einheit wurden auch die hierfr notwendigen Hilfs- und Betriebsstoffe sowie deren Vorketten betrachtet. Fr das Produkt bedeutet dies, die Umweltwirkungen des PVDF-beschichteten Aluminiums, der Schrauben und Klipps, des Bitumens und der Steinwolle werden dem deklarierten Produkt zugerechnet. Ebenso miteinbezogen wird die Herstellung von Verpackungsmaterial (Holz und Kunststoff), Strom und Schmiermittel fr die Produktion im Werk.\n\nModul A5\nEs werden die Umweltwirkungen der Verbrennung der Verpackungsmaterialien Kunststoff und Holz ausgewiesen sowie die Installation auf der Baustelle bercksichtigt.\n\nModul C1\nIn diesem Modul wird die Demontage des Produkts betrachtet. Es wurden die gleichen Aufwendungen, die auch fr die Installation bentigt werden, bercksichtigt.\n\nModul C2\nDas Modul beinhaltet die Transporte zur Abfallbehandlung oder Entsorgung.\n\nModul C3\nDas Modul beinhaltet die Umweltwirkungen durch die Abfallbehandlung (Vorbereitung zum Recycling der Metalle und energetische Verwertung der Kunststoffe und des Bitumens) des Produkts im End-of-Life.\n\nModul C4\nDas Modul beinhaltet die Umweltwirkungen durch die Deponierung der Steinwolle, die im Produkt enthalten ist.\n\nModul D\nDas Modul umfasst den Aufwand des Recyclings und die vermiedenen Umweltlasten fr Aluminium und (Edel-)Stahl, die im Produkt enthalten sind. Daneben werden die vermiedenen Lasten der Energieerzeugung ausgewiesen, die durch die Energiegewinnung aus den brennbaren Materialien resultieren.", "lang": "de"}, {"value": "Scope: \nThis EPD relates to the manufacture, transport, installation and disposal of a representative product with the highest environmental impact (worst case) for a range of products (standing seam roofing and wall cladding system) from Kalzip.The technical properties are presented in chapter 2.3.The production site of the product is Koblenz, Germany, from where the products are delivered directly to the customer's construction sites. \nSystem boundary: \nType of EPD: Cradle to factory gate - with options (module A1–A3, A5, C1–4 and D). \n\nModules A1–A3 \nThe product stage contains the production of the necessary raw materials including all upstream chains as well as the necessary procurement transports. For the production of the declared unit, the necessary auxiliary and operating materials and their upstream chains were also considered. For the product, this means that the environmental impacts of the PVDF-coated aluminium, the screws and clips, the bitumen and rock wool are included in the declared product. Also included is the production of packaging material (wood and plastic), electricity and lubricants for production at the plant. \n\nModule A5 \nThe environmental impacts of the incineration of the packaging materials plastic and wood are shown and the installation on the construction site is taken into account. \n\nModule C1 \nIn this module, the disassembly of the product is considered. \nThe same expenditures that are required for the \ninstallation have been taken into account. \n\nModule C2 \nThe module includes transports for waste treatment or disposal. \n\nModule C3 \nThe module includes the environmental impacts due to the waste treatment (preparation for recycling of metals and energy recovery of plastics and bitumen) of the product in the end of life. \n\nModule C4 \nThe module includes the environmental impacts of landfilling the rock wool contained in the product. \n\nModule D \nThe module includes the effort of recycling and the avoided environmental burdens for aluminium and (stainless) steel contained in the product. In addition, the avoided burdens of energy production resulting from the generation of energy from the combustible materials are shown.", "lang": "en"}], "other": {"anies": [{"name": "referenceToOriginalEPD", "value": {"shortDescription": {"value": "Kalzip® – Stehfalzsystem für Dachdeckungen und Wandbekleidungen aus Aluminium.pdf", "defaultValue": "Kalzip® – Stehfalzsystem für Dachdeckungen und Wandbekleidungen aus Aluminium.pdf", "lstrings": [{"lang": "de", "value": "Kalzip® – Stehfalzsystem für Dachdeckungen und Wandbekleidungen aus Aluminium.pdf"}]}, "type": "source data set", "uuid": {"uuid": "45486cea-db8c-4ea1-b409-0207b692a2b1"}, "refObjectId": "45486cea-db8c-4ea1-b409-0207b692a2b1", "resourceURLs": ["https://oekobaudat.de/OEKOBAU.DAT/resource/sources/45486cea-db8c-4ea1-b409-0207b692a2b1/Kalzip_Stehfalzsystem_fuer_Dachdeckungen_und_Wandbekleidungen_aus_Aluminium_17847.pdf?version=00.03.000"]}}]}}, "validation": {"review": [{"referenceToNameOfReviewerAndInstitution": [{"shortDescription": [{"value": "Institut Bauen und Umwelt e. V.", "lang": "de"}], "type": "contact data set", "refObjectId": "6c991c70-b820-41ba-971e-9aee53dc068c", "uri": "../contacts/6c991c70-b820-41ba-971e-9aee53dc068c.xml"}], "type": "Accredited third party review"}]}, "complianceDeclarations": {"compliance": [{"referenceToComplianceSystem": {"shortDescription": [{"value": "DIN EN 15804+A2", "lang": "de"}], "type": "source data set", "refObjectId": "c0016b33-8cf7-415c-ac6e-deba0d21440d", "uri": "../sources/c0016b33-8cf7-415c-ac6e-deba0d21440d.xml"}}, {"referenceToComplianceSystem": {"shortDescription": [{"value": "ISO 14025", "lang": "de"}], "type": "source data set", "refObjectId": "4f2eb655-6e44-4874-a95a-e28f5442cd4d", "uri": "../sources/4f2eb655-6e44-4874-a95a-e28f5442cd4d.xml"}}]}}, "administrativeInformation": {"commissionerAndGoal": {"referenceToCommissioner": [{"shortDescription": [{"value": "Kalzip GmbH", "lang": "de"}], "type": "contact data set", "refObjectId": "a6e90862-ff2e-4b06-bbfe-1df2360b60f6", "uri": "../contacts/a6e90862-ff2e-4b06-bbfe-1df2360b60f6.xml"}]}, "dataGenerator": {"referenceToPersonOrEntityGeneratingTheDataSet": [{"shortDescription": [{"value": "brands and values GmbH", "lang": "de"}], "type": "contact data set", "refObjectId": "6b539b8a-10e3-4004-8ccc-a79f169aa339", "uri": "../contacts/6b539b8a-10e3-4004-8ccc-a79f169aa339.xml"}]}, "dataEntryBy": {"timeStamp": 1681257600000, "referenceToDataSetFormat": [{"shortDescription": [{"value": "ILCD Format", "lang": "de"}], "type": "source data set", "refObjectId": "a97a0155-0234-4b87-b4ce-a45da52f2a40", "uri": "../sources/a97a0155-0234-4b87-b4ce-a45da52f2a40.xml"}, {"shortDescription": [{"value": "EPD-Datenformaterweiterungen v1.2", "lang": "de"}, {"value": "EPD Data Format Extensions v1.2", "lang": "en"}], "type": "source data set", "refObjectId": "a29449fd-aa2f-4de8-b5d7-4b06b43c6fde", "uri": "../sources/a29449fd-aa2f-4de8-b5d7-4b06b43c6fde.xml"}]}, "publicationAndOwnership": {"dataSetVersion": "00.09.000", "referenceToPrecedingDataSetVersion": [{"shortDescription": [{"value": "Stehfalzsystem für Dachdeckungen und Wandbekleidungen aus Aluminium", "lang": "de"}], "type": "process data set", "refObjectId": "d2056d51-d5fc-4089-9e8f-ba28833ee389", "uri": "../processes/d2056d51-d5fc-4089-9e8f-ba28833ee389.xml"}], "referenceToRegistrationAuthority": {"shortDescription": [{"value": "Institut Bauen und Umwelt e. V.", "lang": "de"}], "type": "contact data set", "refObjectId": "d111dbec-b024-4be5-86c5-752d6eb2cf95", "uri": "../contacts/d111dbec-b024-4be5-86c5-752d6eb2cf95.xml"}, "registrationNumber": "EPD-KAL-20230027-IBC1-DE", "referenceToOwnershipOfDataSet": {"shortDescription": [{"value": "Kalzip GmbH", "lang": "de"}], "type": "contact data set", "refObjectId": "a6e90862-ff2e-4b06-bbfe-1df2360b60f6", "uri": "../contacts/a6e90862-ff2e-4b06-bbfe-1df2360b60f6.xml"}, "copyright": true, "licenseType": "Free of charge for all users and uses", "accessRestrictions": [{"value": "None", "lang": "en"}], "other": {"anies": [{"name": "referenceToPublisher", "value": {"shortDescription": [{"value": "Institut Bauen und Umwelt e. V.", "lang": "de"}], "type": "contact data set", "refObjectId": "d111dbec-b024-4be5-86c5-752d6eb2cf95", "uri": "../contacts/d111dbec-b024-4be5-86c5-752d6eb2cf95.xml"}}]}}}, "exchanges": {"exchange": [{"dataSetInternalID": 0, "referenceToFlowDataSet": {"shortDescription": [{"value": "1m² Stehfalzsystem für Dachdeckungen und Wandbekleidungen aus Aluminium inkl. Verpackung (1m² Stehfalzsystem für Dachdeckungen und Wandbekleidungen aus Aluminium inkl. Verpackung)", "lang": "de"}], "type": "flow data set", "refObjectId": "aea2a3bf-da37-c15d-79cd-2cf74d44ef56", "uri": "../flows/aea2a3bf-da37-c15d-79cd-2cf74d44ef56.xml"}, "meanAmount": 1.0, "referencesToDataSource": {}, "referenceFlow": true, "resolvedFlowVersion": "00.03.000", "resultingflowAmount": 1.0, "flowProperties": [{"name": [{"lang": "en", "value": "Area"}, {"lang": "de", "value": "Fläche"}], "uuid": "93a60a56-a3c8-19da-a746-0800200c9a66", "referenceFlowProperty": true, "meanValue": 1.0, "referenceUnit": "qm", "unitGroupUUID": "c20a03d7-bd90-4569-bc94-66cfd364dfc8"}], "materialProperties": [{"name": "grammage", "value": "13.97", "unit": "kg/m^2", "unitDescription": "kilograms per square meter"}, {"name": "layer thickness", "value": "0.265", "unit": "m", "unitDescription": "meters"}, {"name": "conversion factor to 1 kg", "value": "0.07", "unit": "-", "unitDescription": "Without unit"}], "typeOfFlow": "Product flow", "classification": {"classHierarchy": "Metalle / Aluminium / Aluminiumprofil", "name": "OEKOBAU.DAT"}}, {"dataSetInternalID": 1, "referenceToFlowDataSet": {"shortDescription": [{"value": "Erneuerbare Primärenergie als Energieträger (PERE)", "lang": "de"}, {"value": "Renewable primary energy as energy carrier (PERE)", "lang": "en"}], "type": "flow data set", "refObjectId": "20f32be5-0398-4288-9b6d-accddd195317", "uri": "../flows/20f32be5-0398-4288-9b6d-accddd195317.xml"}, "exchange direction": "INPUT", "other": {"anies": [{"name": "referenceToUnitGroupDataSet", "value": {"shortDescription": [{"value": "MJ", "lang": "de"}], "type": "unit group data set", "refObjectId": "93a60a57-a3c8-11da-a746-0800200c9a66", "uri": "../unitgroups/93a60a57-a3c8-11da-a746-0800200c9a66.xml"}}, {"value": "72.77682", "module": "A1-A3"}, {"value": "3.14548", "module": "A5"}, {"value": "0.00338", "module": "C1"}, {"value": "0.0811", "module": "C2"}, {"value": "0.563", "module": "C3"}, {"value": "0.24", "module": "C4"}, {"value": "-32.9", "module": "D"}]}, "resolvedFlowVersion": "38.00.000", "flowProperties": [], "typeOfFlow": "Other flow", "classification": {"classHierarchy": "Quantities", "name": "GaBiCategories"}}, {"dataSetInternalID": 2, "referenceToFlowDataSet": {"shortDescription": [{"value": "Erneuerbare Primärenergie zur stofflichen Nutzung (PERM)", "lang": "de"}, {"value": "Renewable primary energy resources as material utilization (PERM)", "lang": "en"}], "type": "flow data set", "refObjectId": "fb3ec0de-548d-4508-aea5-00b73bf6f702", "uri": "../flows/fb3ec0de-548d-4508-aea5-00b73bf6f702.xml"}, "exchange direction": "INPUT", "other": {"anies": [{"name": "referenceToUnitGroupDataSet", "value": {"shortDescription": [{"value": "MJ", "lang": "de"}], "type": "unit group data set", "refObjectId": "93a60a57-a3c8-11da-a746-0800200c9a66", "uri": "../unitgroups/93a60a57-a3c8-11da-a746-0800200c9a66.xml"}}, {"value": "3.12318", "module": "A1-A3"}, {"value": "-3.12318", "module": "A5"}, {"value": "0", "module": "C1"}, {"value": "0", "module": "C2"}, {"value": "0", "module": "C3"}, {"value": "0", "module": "C4"}, {"value": "0", "module": "D"}]}, "resolvedFlowVersion": "38.00.000", "flowProperties": [], "typeOfFlow": "Other flow", "classification": {"classHierarchy": "Quantities", "name": "GaBiCategories"}}, {"dataSetInternalID": 3, "referenceToFlowDataSet": {"shortDescription": [{"value": "Total erneuerbare Primärenergie (PERT)", "lang": "de"}, {"value": "Total use of renewable primary energy resources (PERT)", "lang": "en"}], "type": "flow data set", "refObjectId": "53f97275-fa8a-4cdd-9024-65936002acd0", "uri": "../flows/53f97275-fa8a-4cdd-9024-65936002acd0.xml"}, "exchange direction": "INPUT", "other": {"anies": [{"name": "referenceToUnitGroupDataSet", "value": {"shortDescription": [{"value": "MJ", "lang": "de"}], "type": "unit group data set", "refObjectId": "93a60a57-a3c8-11da-a746-0800200c9a66", "uri": "../unitgroups/93a60a57-a3c8-11da-a746-0800200c9a66.xml"}}, {"value": "75.9", "module": "A1-A3"}, {"value": "0.0223", "module": "A5"}, {"value": "0.00338", "module": "C1"}, {"value": "0.0811", "module": "C2"}, {"value": "0.563", "module": "C3"}, {"value": "0.24", "module": "C4"}, {"value": "-32.9", "module": "D"}]}, "resolvedFlowVersion": "38.00.000", "flowProperties": [], "typeOfFlow": "Other flow", "classification": {"classHierarchy": "Quantities / Environmental quantities / EPD EN 15804 / LCI indicators", "name": "GaBiCategories"}}, {"dataSetInternalID": 4, "referenceToFlowDataSet": {"shortDescription": [{"value": "Nicht-erneuerbare Primärenergie als Energieträger (PENRE)", "lang": "de"}, {"value": "Non renewable primary energy as energy carrier (PENRE)", "lang": "en"}], "type": "flow data set", "refObjectId": "ac857178-2b45-46ec-892a-a9a4332f0372", "uri": "../flows/ac857178-2b45-46ec-892a-a9a4332f0372.xml"}, "exchange direction": "INPUT", "other": {"anies": [{"name": "referenceToUnitGroupDataSet", "value": {"shortDescription": [{"value": "MJ", "lang": "de"}], "type": "unit group data set", "refObjectId": "93a60a57-a3c8-11da-a746-0800200c9a66", "uri": "../unitgroups/93a60a57-a3c8-11da-a746-0800200c9a66.xml"}}, {"value": "323.159980975", "module": "A1-A3"}, {"value": "1.234571025", "module": "A5"}, {"value": "0.0234", "module": "C1"}, {"value": "1.18", "module": "C2"}, {"value": "36.165448", "module": "C3"}, {"value": "1.6", "module": "C4"}, {"value": "-70.9", "module": "D"}]}, "resolvedFlowVersion": "38.00.000", "flowProperties": [], "typeOfFlow": "Other flow", "classification": {"classHierarchy": "Quantities", "name": "GaBiCategories"}}, {"dataSetInternalID": 5, "referenceToFlowDataSet": {"shortDescription": [{"value": "Nicht-erneuerbare Primärenergie zur stofflichen Nutzung (PENRM)", "lang": "de"}, {"value": "Non renewable primary energy as material utilization (PENRM)", "lang": "en"}], "type": "flow data set", "refObjectId": "1421caa0-679d-4bf4-b282-0eb850ccae27", "uri": "../flows/1421caa0-679d-4bf4-b282-0eb850ccae27.xml"}, "exchange direction": "INPUT", "other": {"anies": [{"name": "referenceToUnitGroupDataSet", "value": {"shortDescription": [{"value": "MJ", "lang": "de"}], "type": "unit group data set", "refObjectId": "93a60a57-a3c8-11da-a746-0800200c9a66", "uri": "../unitgroups/93a60a57-a3c8-11da-a746-0800200c9a66.xml"}}, {"value": "35.840019025", "module": "A1-A3"}, {"value": "-1.114571025", "module": "A5"}, {"value": "0", "module": "C1"}, {"value": "0", "module": "C2"}, {"value": "-34.725448", "module": "C3"}, {"value": "0", "module": "C4"}, {"value": "0", "module": "D"}]}, "resolvedFlowVersion": "38.00.000", "flowProperties": [], "typeOfFlow": "Other flow", "classification": {"classHierarchy": "Quantities", "name": "GaBiCategories"}}, {"dataSetInternalID": 6, "referenceToFlowDataSet": {"shortDescription": [{"value": "Total nicht erneuerbare Primärenergie (PENRT)", "lang": "de"}, {"value": "Total use of non renewable primary energy resources (PENRT)", "lang": "en"}], "type": "flow data set", "refObjectId": "06159210-646b-4c8d-8583-da9b3b95a6c1", "uri": "../flows/06159210-646b-4c8d-8583-da9b3b95a6c1.xml"}, "exchange direction": "INPUT", "other": {"anies": [{"name": "referenceToUnitGroupDataSet", "value": {"shortDescription": [{"value": "MJ", "lang": "de"}], "type": "unit group data set", "refObjectId": "93a60a57-a3c8-11da-a746-0800200c9a66", "uri": "../unitgroups/93a60a57-a3c8-11da-a746-0800200c9a66.xml"}}, {"value": "359", "module": "A1-A3"}, {"value": "0.12", "module": "A5"}, {"value": "0.0234", "module": "C1"}, {"value": "1.18", "module": "C2"}, {"value": "1.44", "module": "C3"}, {"value": "1.6", "module": "C4"}, {"value": "-70.9", "module": "D"}]}, "resolvedFlowVersion": "38.00.000", "flowProperties": [], "typeOfFlow": "Other flow", "classification": {"classHierarchy": "Quantities / Environmental quantities / EPD EN 15804 / LCI indicators", "name": "GaBiCategories"}}, {"dataSetInternalID": 7, "referenceToFlowDataSet": {"shortDescription": [{"value": "Einsatz von Sekundärstoffen (SM)", "lang": "de"}, {"value": "Use of secondary material (SM)", "lang": "en"}], "type": "flow data set", "refObjectId": "c6a1f35f-2d09-4f54-8dfb-97e502e1ce92", "uri": "../flows/c6a1f35f-2d09-4f54-8dfb-97e502e1ce92.xml"}, "exchange direction": "INPUT", "other": {"anies": [{"name": "referenceToUnitGroupDataSet", "value": {"shortDescription": [{"value": "kg", "lang": "de"}], "type": "unit group data set", "refObjectId": "ad38d542-3fe9-439d-9b95-2f5f7752acaf", "uri": "../unitgroups/ad38d542-3fe9-439d-9b95-2f5f7752acaf.xml"}}, {"value": "3.08", "module": "A1-A3"}, {"value": "0", "module": "A5"}, {"value": "0", "module": "C1"}, {"value": "0", "module": "C2"}, {"value": "0", "module": "C3"}, {"value": "0", "module": "C4"}, {"value": "0.695", "module": "D"}]}, "resolvedFlowVersion": "38.00.000", "flowProperties": [], "typeOfFlow": "Other flow", "classification": {"classHierarchy": "Quantities / Environmental quantities / EPD EN 15804 / LCI indicators", "name": "GaBiCategories"}}, {"dataSetInternalID": 8, "referenceToFlowDataSet": {"shortDescription": [{"value": "Erneuerbare Sekundärbrennstoffe (RSF)", "lang": "de"}, {"value": "Use of renewable secondary fuels (RSF)", "lang": "en"}], "type": "flow data set", "refObjectId": "64333088-a55f-4aa2-9a31-c10b07816787", "uri": "../flows/64333088-a55f-4aa2-9a31-c10b07816787.xml"}, "exchange direction": "INPUT", "other": {"anies": [{"name": "referenceToUnitGroupDataSet", "value": {"shortDescription": [{"value": "MJ", "lang": "de"}], "type": "unit group data set", "refObjectId": "93a60a57-a3c8-11da-a746-0800200c9a66", "uri": "../unitgroups/93a60a57-a3c8-11da-a746-0800200c9a66.xml"}}, {"value": "0", "module": "A1-A3"}, {"value": "0", "module": "A5"}, {"value": "0", "module": "C1"}, {"value": "0", "module": "C2"}, {"value": "0", "module": "C3"}, {"value": "0", "module": "C4"}, {"value": "0", "module": "D"}]}, "resolvedFlowVersion": "38.00.000", "flowProperties": [], "typeOfFlow": "Other flow", "classification": {"classHierarchy": "Quantities / Environmental quantities / EPD EN 15804 / LCI indicators", "name": "GaBiCategories"}}, {"dataSetInternalID": 9, "referenceToFlowDataSet": {"shortDescription": [{"value": "Nicht erneuerbare Sekundärbrennstoffe (NRSF)", "lang": "de"}, {"value": "Use of non renewable secondary fuels (NRSF)", "lang": "en"}], "type": "flow data set", "refObjectId": "89def144-d39a-4287-b86f-efde453ddcb2", "uri": "../flows/89def144-d39a-4287-b86f-efde453ddcb2.xml"}, "exchange direction": "INPUT", "other": {"anies": [{"name": "referenceToUnitGroupDataSet", "value": {"shortDescription": [{"value": "MJ", "lang": "de"}], "type": "unit group data set", "refObjectId": "93a60a57-a3c8-11da-a746-0800200c9a66", "uri": "../unitgroups/93a60a57-a3c8-11da-a746-0800200c9a66.xml"}}, {"value": "0", "module": "A1-A3"}, {"value": "0", "module": "A5"}, {"value": "0", "module": "C1"}, {"value": "0", "module": "C2"}, {"value": "0", "module": "C3"}, {"value": "0", "module": "C4"}, {"value": "0", "module": "D"}]}, "resolvedFlowVersion": "38.00.000", "flowProperties": [], "typeOfFlow": "Other flow", "classification": {"classHierarchy": "Quantities / Environmental quantities / EPD EN 15804 / LCI indicators", "name": "GaBiCategories"}}, {"dataSetInternalID": 10, "referenceToFlowDataSet": {"shortDescription": [{"value": "Einsatz von Süßwasserressourcen (FW)", "lang": "de"}, {"value": "Use of net fresh water (FW)", "lang": "en"}], "type": "flow data set", "refObjectId": "3cf952c8-f3a4-461d-8c96-96456ca62246", "uri": "../flows/3cf952c8-f3a4-461d-8c96-96456ca62246.xml"}, "exchange direction": "INPUT", "other": {"anies": [{"name": "referenceToUnitGroupDataSet", "value": {"shortDescription": [{"value": "m^3", "lang": "de"}], "type": "unit group data set", "refObjectId": "cd950537-0a98-4044-9ba7-9f9a68d0a504", "uri": "../unitgroups/cd950537-0a98-4044-9ba7-9f9a68d0a504.xml"}}, {"value": "0.147", "module": "A1-A3"}, {"value": "0.000949", "module": "A5"}, {"value": "5.12E-06", "module": "C1"}, {"value": "9.37E-05", "module": "C2"}, {"value": "0.00735", "module": "C3"}, {"value": "0.000406", "module": "C4"}, {"value": "-0.0772", "module": "D"}]}, "resolvedFlowVersion": "38.00.000", "flowProperties": [], "typeOfFlow": "Other flow", "classification": {"classHierarchy": "Quantities / Environmental quantities / EPD EN 15804 / LCI indicators", "name": "GaBiCategories"}}, {"dataSetInternalID": 11, "referenceToFlowDataSet": {"shortDescription": [{"value": "Gefährlicher Abfall zur Deponie (HWD)", "lang": "de"}, {"value": "Hazardous waste disposed (HWD)", "lang": "en"}], "type": "flow data set", "refObjectId": "430f9e0f-59b2-46a0-8e0d-55e0e84948fc", "uri": "../flows/430f9e0f-59b2-46a0-8e0d-55e0e84948fc.xml"}, "exchange direction": "OUTPUT", "other": {"anies": [{"name": "referenceToUnitGroupDataSet", "value": {"shortDescription": [{"value": "kg", "lang": "de"}], "type": "unit group data set", "refObjectId": "ad38d542-3fe9-439d-9b95-2f5f7752acaf", "uri": "../unitgroups/ad38d542-3fe9-439d-9b95-2f5f7752acaf.xml"}}, {"value": "6.77E-08", "module": "A1-A3"}, {"value": "9E-12", "module": "A5"}, {"value": "1.67E-12", "module": "C1"}, {"value": "6.22E-12", "module": "C2"}, {"value": "1.49E-10", "module": "C3"}, {"value": "8.24E-11", "module": "C4"}, {"value": "-4.02E-06", "module": "D"}]}, "resolvedFlowVersion": "38.00.000", "flowProperties": [], "typeOfFlow": "Other flow", "classification": {"classHierarchy": "Quantities / Environmental quantities / EPD EN 15804 / LCI indicators", "name": "GaBiCategories"}}, {"dataSetInternalID": 12, "referenceToFlowDataSet": {"shortDescription": [{"value": "Entsorgter nicht gefährlicher Abfall (NHWD)", "lang": "de"}, {"value": "Non hazardous waste disposed (NHWD)", "lang": "en"}], "type": "flow data set", "refObjectId": "b29ef66b-e286-4afa-949f-62f1a7b4d7fa", "uri": "../flows/b29ef66b-e286-4afa-949f-62f1a7b4d7fa.xml"}, "exchange direction": "OUTPUT", "other": {"anies": [{"name": "referenceToUnitGroupDataSet", "value": {"shortDescription": [{"value": "kg", "lang": "de"}], "type": "unit group data set", "refObjectId": "ad38d542-3fe9-439d-9b95-2f5f7752acaf", "uri": "../unitgroups/ad38d542-3fe9-439d-9b95-2f5f7752acaf.xml"}}, {"value": "5.75", "module": "A1-A3"}, {"value": "0.0026", "module": "A5"}, {"value": "4.98E-06", "module": "C1"}, {"value": "0.000191", "module": "C2"}, {"value": "0.016", "module": "C3"}, {"value": "8.21", "module": "C4"}, {"value": "-1.46", "module": "D"}]}, "resolvedFlowVersion": "38.00.000", "flowProperties": [], "typeOfFlow": "Other flow", "classification": {"classHierarchy": "Quantities / Environmental quantities / EPD EN 15804 / LCI indicators", "name": "GaBiCategories"}}, {"dataSetInternalID": 13, "referenceToFlowDataSet": {"shortDescription": [{"value": "Entsorgter radioaktiver Abfall (RWD)", "lang": "de"}, {"value": "Radioactive waste disposed (RWD)", "lang": "en"}], "type": "flow data set", "refObjectId": "3449546e-52ad-4b39-b809-9fb77cea8ff6", "uri": "../flows/3449546e-52ad-4b39-b809-9fb77cea8ff6.xml"}, "exchange direction": "OUTPUT", "other": {"anies": [{"name": "referenceToUnitGroupDataSet", "value": {"shortDescription": [{"value": "kg", "lang": "de"}], "type": "unit group data set", "refObjectId": "ad38d542-3fe9-439d-9b95-2f5f7752acaf", "uri": "../unitgroups/ad38d542-3fe9-439d-9b95-2f5f7752acaf.xml"}}, {"value": "0.0132", "module": "A1-A3"}, {"value": "8.38E-06", "module": "A5"}, {"value": "3.89E-06", "module": "C1"}, {"value": "2.18E-06", "module": "C2"}, {"value": "0.000157", "module": "C3"}, {"value": "1.78E-05", "module": "C4"}, {"value": "-0.00483", "module": "D"}]}, "resolvedFlowVersion": "38.00.000", "flowProperties": [], "typeOfFlow": "Other flow", "classification": {"classHierarchy": "Quantities / Environmental quantities / EPD EN 15804 / LCI indicators", "name": "GaBiCategories"}}, {"dataSetInternalID": 14, "referenceToFlowDataSet": {"shortDescription": [{"value": "Komponenten für die Wiederverwendung (CRU)", "lang": "de"}, {"value": "Components for re-use (CRU)", "lang": "en"}], "type": "flow data set", "refObjectId": "a2b32f97-3fc7-4af2-b209-525bc6426f33", "uri": "../flows/a2b32f97-3fc7-4af2-b209-525bc6426f33.xml"}, "exchange direction": "OUTPUT", "other": {"anies": [{"name": "referenceToUnitGroupDataSet", "value": {"shortDescription": [{"value": "kg", "lang": "de"}], "type": "unit group data set", "refObjectId": "ad38d542-3fe9-439d-9b95-2f5f7752acaf", "uri": "../unitgroups/ad38d542-3fe9-439d-9b95-2f5f7752acaf.xml"}}, {"value": "0", "module": "A1-A3"}, {"value": "0", "module": "A5"}, {"value": "0", "module": "C1"}, {"value": "0", "module": "C2"}, {"value": "0", "module": "C3"}, {"value": "0", "module": "C4"}, {"value": "0", "module": "D"}]}, "resolvedFlowVersion": "38.00.000", "flowProperties": [], "typeOfFlow": "Other flow", "classification": {"classHierarchy": "Quantities / Environmental quantities / EPD EN 15804 / LCI indicators", "name": "GaBiCategories"}}, {"dataSetInternalID": 15, "referenceToFlowDataSet": {"shortDescription": [{"value": "Stoffe zum Recycling (MFR)", "lang": "de"}, {"value": "Materials for recycling (MFR)", "lang": "en"}], "type": "flow data set", "refObjectId": "d7fe48a5-4103-49c8-9aae-b0b5dfdbd6ae", "uri": "../flows/d7fe48a5-4103-49c8-9aae-b0b5dfdbd6ae.xml"}, "exchange direction": "OUTPUT", "other": {"anies": [{"name": "referenceToUnitGroupDataSet", "value": {"shortDescription": [{"value": "kg", "lang": "de"}], "type": "unit group data set", "refObjectId": "ad38d542-3fe9-439d-9b95-2f5f7752acaf", "uri": "../unitgroups/ad38d542-3fe9-439d-9b95-2f5f7752acaf.xml"}}, {"value": "0", "module": "A1-A3"}, {"value": "0", "module": "A5"}, {"value": "0", "module": "C1"}, {"value": "0", "module": "C2"}, {"value": "4.16", "module": "C3"}, {"value": "0", "module": "C4"}, {"value": "0", "module": "D"}]}, "resolvedFlowVersion": "38.00.000", "flowProperties": [], "typeOfFlow": "Other flow", "classification": {"classHierarchy": "Quantities / Environmental quantities / EPD EN 15804 / LCI indicators", "name": "GaBiCategories"}}, {"dataSetInternalID": 16, "referenceToFlowDataSet": {"shortDescription": [{"value": "Stoffe für die Energierückgewinnung (MER)", "lang": "de"}, {"value": "Materials for energy recovery (MER)", "lang": "en"}], "type": "flow data set", "refObjectId": "59a9181c-3aaf-46ee-8b13-2b3723b6e447", "uri": "../flows/59a9181c-3aaf-46ee-8b13-2b3723b6e447.xml"}, "exchange direction": "OUTPUT", "other": {"anies": [{"name": "referenceToUnitGroupDataSet", "value": {"shortDescription": [{"value": "kg", "lang": "de"}], "type": "unit group data set", "refObjectId": "ad38d542-3fe9-439d-9b95-2f5f7752acaf", "uri": "../unitgroups/ad38d542-3fe9-439d-9b95-2f5f7752acaf.xml"}}, {"value": "0", "module": "A1-A3"}, {"value": "0", "module": "A5"}, {"value": "0", "module": "C1"}, {"value": "0", "module": "C2"}, {"value": "0", "module": "C3"}, {"value": "0", "module": "C4"}, {"value": "0", "module": "D"}]}, "resolvedFlowVersion": "38.00.000", "flowProperties": [], "typeOfFlow": "Other flow", "classification": {"classHierarchy": "Quantities / Environmental quantities / EPD EN 15804 / LCI indicators", "name": "GaBiCategories"}}, {"dataSetInternalID": 17, "referenceToFlowDataSet": {"shortDescription": [{"value": "Exportierte elektrische Energie (EEE)", "lang": "de"}, {"value": "Exported electrical energy (EEE)", "lang": "en"}], "type": "flow data set", "refObjectId": "4da0c987-2b76-40d6-9e9e-82a017aaaf29", "uri": "../flows/4da0c987-2b76-40d6-9e9e-82a017aaaf29.xml"}, "exchange direction": "OUTPUT", "other": {"anies": [{"name": "referenceToUnitGroupDataSet", "value": {"shortDescription": [{"value": "MJ", "lang": "de"}], "type": "unit group data set", "refObjectId": "93a60a57-a3c8-11da-a746-0800200c9a66", "uri": "../unitgroups/93a60a57-a3c8-11da-a746-0800200c9a66.xml"}}, {"value": "0", "module": "A1-A3"}, {"value": "0.625", "module": "A5"}, {"value": "0", "module": "C1"}, {"value": "0", "module": "C2"}, {"value": "3.94", "module": "C3"}, {"value": "0", "module": "C4"}, {"value": "0", "module": "D"}]}, "resolvedFlowVersion": "38.00.000", "flowProperties": [], "typeOfFlow": "Other flow", "classification": {"classHierarchy": "Quantities / Environmental quantities / EPD EN 15804 / LCI indicators", "name": "GaBiCategories"}}, {"dataSetInternalID": 18, "referenceToFlowDataSet": {"shortDescription": [{"value": "Exportierte thermische Energie (EET)", "lang": "de"}, {"value": "Exported thermal energy (EET)", "lang": "en"}], "type": "flow data set", "refObjectId": "98daf38a-7a79-46d3-9a37-2b7bd0955810", "uri": "../flows/98daf38a-7a79-46d3-9a37-2b7bd0955810.xml"}, "exchange direction": "OUTPUT", "other": {"anies": [{"name": "referenceToUnitGroupDataSet", "value": {"shortDescription": [{"value": "MJ", "lang": "de"}], "type": "unit group data set", "refObjectId": "93a60a57-a3c8-11da-a746-0800200c9a66", "uri": "../unitgroups/93a60a57-a3c8-11da-a746-0800200c9a66.xml"}}, {"value": "0", "module": "A1-A3"}, {"value": "1.12", "module": "A5"}, {"value": "0", "module": "C1"}, {"value": "0", "module": "C2"}, {"value": "7.07", "module": "C3"}, {"value": "0", "module": "C4"}, {"value": "0", "module": "D"}]}, "resolvedFlowVersion": "38.00.000", "flowProperties": [], "typeOfFlow": "Other flow", "classification": {"classHierarchy": "Quantities / Environmental quantities / EPD EN 15804 / LCI indicators", "name": "GaBiCategories"}}]}, "LCIAResults": {"LCIAResult": [{"referenceToLCIAMethodDataSet": {"shortDescription": [{"value": "Globales Erwärmungspotenzial total (GWP-total)", "lang": "de"}, {"value": "Global Warming Potential total (GWP-total)", "lang": "en"}], "type": "LCIA method data set", "refObjectId": "6a37f984-a4b3-458a-a20a-64418c145fa2", "uri": "../lciamethods/6a37f984-a4b3-458a-a20a-64418c145fa2.xml"}, "other": {"anies": [{"name": "referenceToUnitGroupDataSet", "value": {"shortDescription": [{"value": "kg CO_(2)-Äq.", "lang": "de"}], "type": "unit group data set", "refObjectId": "1ebf3012-d0db-4de2-aefd-ef30cedb0be1", "uri": "../unitgroups/1ebf3012-d0db-4de2-aefd-ef30cedb0be1.xml"}}, {"value": "24.5", "module": "A1-A3"}, {"value": "0.377", "module": "A5"}, {"value": "0.0011", "module": "C1"}, {"value": "0.0896", "module": "C2"}, {"value": "3.27", "module": "C3"}, {"value": "0.123", "module": "C4"}, {"value": "-5.35", "module": "D"}]}}, {"referenceToLCIAMethodDataSet": {"shortDescription": [{"value": "Globales Erwärmungspotenzial fossil (GWP-fossil)", "lang": "de"}, {"value": "Global Warming Potential fossil fuels (GWP-fossil)", "lang": "en"}], "type": "LCIA method data set", "refObjectId": "5f635281-343e-44fb-83df-1971b155e6b6", "uri": "../lciamethods/5f635281-343e-44fb-83df-1971b155e6b6.xml"}, "other": {"anies": [{"name": "referenceToUnitGroupDataSet", "value": {"shortDescription": [{"value": "kg CO_(2)-Äq.", "lang": "de"}], "type": "unit group data set", "refObjectId": "1ebf3012-d0db-4de2-aefd-ef30cedb0be1", "uri": "../unitgroups/1ebf3012-d0db-4de2-aefd-ef30cedb0be1.xml"}}, {"value": "24.8", "module": "A1-A3"}, {"value": "0.0897", "module": "A5"}, {"value": "0.0011", "module": "C1"}, {"value": "0.089", "module": "C2"}, {"value": "3.27", "module": "C3"}, {"value": "0.122", "module": "C4"}, {"value": "-5.35", "module": "D"}]}}, {"referenceToLCIAMethodDataSet": {"shortDescription": [{"value": "Globales Erwärmungspotenzial biogen (GWP-biogenic)", "lang": "de"}, {"value": "Global Warming Potential biogenic (GWP-biogenic)", "lang": "en"}], "type": "LCIA method data set", "refObjectId": "2356e1ab-0185-4db5-86e5-16de51c7485c", "uri": "../lciamethods/2356e1ab-0185-4db5-86e5-16de51c7485c.xml"}, "other": {"anies": [{"name": "referenceToUnitGroupDataSet", "value": {"shortDescription": [{"value": "kg CO_(2)-Äq.", "lang": "de"}], "type": "unit group data set", "refObjectId": "1ebf3012-d0db-4de2-aefd-ef30cedb0be1", "uri": "../unitgroups/1ebf3012-d0db-4de2-aefd-ef30cedb0be1.xml"}}, {"value": "-0.287", "module": "A1-A3"}, {"value": "0.287", "module": "A5"}, {"value": "0", "module": "C1"}, {"value": "0", "module": "C2"}, {"value": "0", "module": "C3"}, {"value": "0", "module": "C4"}, {"value": "0", "module": "D"}]}}, {"referenceToLCIAMethodDataSet": {"shortDescription": [{"value": "Globales Erwärmungspotenzial luluc (GWP-luluc)", "lang": "de"}, {"value": "Global Warming Potential luluc (GWP-luluc)", "lang": "en"}], "type": "LCIA method data set", "refObjectId": "4331bbdb-978a-490d-8707-eeb047f01a55", "uri": "../lciamethods/4331bbdb-978a-490d-8707-eeb047f01a55.xml"}, "other": {"anies": [{"name": "referenceToUnitGroupDataSet", "value": {"shortDescription": [{"value": "kg CO_(2)-Äq.", "lang": "de"}], "type": "unit group data set", "refObjectId": "1ebf3012-d0db-4de2-aefd-ef30cedb0be1", "uri": "../unitgroups/1ebf3012-d0db-4de2-aefd-ef30cedb0be1.xml"}}, {"value": "0.00775", "module": "A1-A3"}, {"value": "1.17E-05", "module": "A5"}, {"value": "7.16E-08", "module": "C1"}, {"value": "0.000601", "module": "C2"}, {"value": "1.41E-05", "module": "C3"}, {"value": "0.000226", "module": "C4"}, {"value": "-0.00116", "module": "D"}]}}, {"referenceToLCIAMethodDataSet": {"shortDescription": [{"value": "Abbau Potential der stratosphärischen Ozonschicht (ODP)", "lang": "de"}, {"value": "Depletion potential of the stratospheric ozone layer (ODP)", "lang": "en"}], "type": "LCIA method data set", "refObjectId": "b5c629d6-def3-11e6-bf01-fe55135034f3", "uri": "../lciamethods/b5c629d6-def3-11e6-bf01-fe55135034f3.xml"}, "other": {"anies": [{"name": "referenceToUnitGroupDataSet", "value": {"shortDescription": [{"value": "kg CFC11-Äq.", "lang": "de"}], "type": "unit group data set", "refObjectId": "d9e957c9-7309-4474-bf3a-7777df6c4e5b", "uri": "../unitgroups/d9e957c9-7309-4474-bf3a-7777df6c4e5b.xml"}}, {"value": "3.79E-07", "module": "A1-A3"}, {"value": "3.83E-14", "module": "A5"}, {"value": "1.09E-14", "module": "C1"}, {"value": "8.76E-15", "module": "C2"}, {"value": "8.37E-13", "module": "C3"}, {"value": "2.87E-13", "module": "C4"}, {"value": "4.75E-11", "module": "D"}]}}, {"referenceToLCIAMethodDataSet": {"shortDescription": [{"value": "Versauerungspotenzial von Boden und Wasser (AP)", "lang": "de"}, {"value": "Acidification potential of land and water (AP)", "lang": "en"}], "type": "LCIA method data set", "refObjectId": "b5c611c6-def3-11e6-bf01-fe55135034f3", "uri": "../lciamethods/b5c611c6-def3-11e6-bf01-fe55135034f3.xml"}, "other": {"anies": [{"name": "referenceToUnitGroupDataSet", "value": {"shortDescription": [{"value": "mol H^(+)-Äq.", "lang": "de"}], "type": "unit group data set", "refObjectId": "42e089ac-92bf-4bf2-8ca1-5fc40d18f2ed", "uri": "../unitgroups/42e089ac-92bf-4bf2-8ca1-5fc40d18f2ed.xml"}}, {"value": "0.136", "module": "A1-A3"}, {"value": "6E-05", "module": "A5"}, {"value": "1.62E-06", "module": "C1"}, {"value": "0.000316", "module": "C2"}, {"value": "0.00121", "module": "C3"}, {"value": "0.000868", "module": "C4"}, {"value": "-0.0246", "module": "D"}]}}, {"referenceToLCIAMethodDataSet": {"shortDescription": [{"value": "Eutrophierungspotenzial Süßwasser (EP-freshwater)", "lang": "de"}, {"value": "Eutrophication potential aquatic freshwater (EP-freshwater)", "lang": "en"}], "type": "LCIA method data set", "refObjectId": "b53ec18f-7377-4ad3-86eb-cc3f4f276b2b", "uri": "../lciamethods/b53ec18f-7377-4ad3-86eb-cc3f4f276b2b.xml"}, "other": {"anies": [{"name": "referenceToUnitGroupDataSet", "value": {"shortDescription": [{"value": "kg P-Äq.", "lang": "de"}], "type": "unit group data set", "refObjectId": "0429039d-a61d-4590-ba67-aa4a20a810a1", "uri": "../unitgroups/0429039d-a61d-4590-ba67-aa4a20a810a1.xml"}}, {"value": "2.26E-05", "module": "A1-A3"}, {"value": "1.28E-08", "module": "A5"}, {"value": "4.95E-10", "module": "C1"}, {"value": "3.19E-07", "module": "C2"}, {"value": "1.78E-07", "module": "C3"}, {"value": "2.07E-07", "module": "C4"}, {"value": "-3.11E-06", "module": "D"}]}}, {"referenceToLCIAMethodDataSet": {"shortDescription": [{"value": "Eutrophierungspotenzial Salzwasser (EP-marine)", "lang": "de"}, {"value": "Eutrophication potential aquatic marine (EP-marine)", "lang": "en"}], "type": "LCIA method data set", "refObjectId": "b5c619fa-def3-11e6-bf01-fe55135034f3", "uri": "../lciamethods/b5c619fa-def3-11e6-bf01-fe55135034f3.xml"}, "other": {"anies": [{"name": "referenceToUnitGroupDataSet", "value": {"shortDescription": [{"value": "kg N-Äq.", "lang": "de"}], "type": "unit group data set", "refObjectId": "d05bb823-ecdf-4686-8c40-bf1d9257859f", "uri": "../unitgroups/d05bb823-ecdf-4686-8c40-bf1d9257859f.xml"}}, {"value": "0.017", "module": "A1-A3"}, {"value": "1.94E-05", "module": "A5"}, {"value": "4.43E-07", "module": "C1"}, {"value": "0.000146", "module": "C2"}, {"value": "0.000531", "module": "C3"}, {"value": "0.000222", "module": "C4"}, {"value": "-0.00325", "module": "D"}]}}, {"referenceToLCIAMethodDataSet": {"shortDescription": [{"value": "Eutrophierungspotenzial Land (EP-terrestrial)", "lang": "de"}, {"value": "Eutrophication potential terrestrial (EP-terrestrial)", "lang": "en"}], "type": "LCIA method data set", "refObjectId": "b5c614d2-def3-11e6-bf01-fe55135034f3", "uri": "../lciamethods/b5c614d2-def3-11e6-bf01-fe55135034f3.xml"}, "other": {"anies": [{"name": "referenceToUnitGroupDataSet", "value": {"shortDescription": [{"value": "mol N-Äq.", "lang": "de"}], "type": "unit group data set", "refObjectId": "71b4d617-0ec9-4d3f-b65e-e438940c2401", "uri": "../unitgroups/71b4d617-0ec9-4d3f-b65e-e438940c2401.xml"}}, {"value": "0.348", "module": "A1-A3"}, {"value": "0.000284", "module": "A5"}, {"value": "4.74E-06", "module": "C1"}, {"value": "0.00163", "module": "C2"}, {"value": "0.0063", "module": "C3"}, {"value": "0.00244", "module": "C4"}, {"value": "-0.0353", "module": "D"}]}}, {"referenceToLCIAMethodDataSet": {"shortDescription": [{"value": "Bildungspotential für troposphärisches Ozon (POCP)", "lang": "de"}, {"value": "Formation potential of tropospheric ozone photochemical oxidants (POCP)", "lang": "en"}], "type": "LCIA method data set", "refObjectId": "b5c610fe-def3-11e6-bf01-fe55135034f3", "uri": "../lciamethods/b5c610fe-def3-11e6-bf01-fe55135034f3.xml"}, "other": {"anies": [{"name": "referenceToUnitGroupDataSet", "value": {"shortDescription": [{"value": "kg NMVOC-Äq.", "lang": "de"}], "type": "unit group data set", "refObjectId": "d27c25f8-fbc1-44c6-b47b-4adbae4199c6", "uri": "../unitgroups/d27c25f8-fbc1-44c6-b47b-4adbae4199c6.xml"}}, {"value": "0.0534", "module": "A1-A3"}, {"value": "5.11E-05", "module": "A5"}, {"value": "1.25E-06", "module": "C1"}, {"value": "0.000285", "module": "C2"}, {"value": "0.00138", "module": "C3"}, {"value": "0.000674", "module": "C4"}, {"value": "-0.00996", "module": "D"}]}}, {"referenceToLCIAMethodDataSet": {"shortDescription": [{"value": "Potenzial für den abiotischen Abbau nicht fossiler Ressourcen (ADPE)", "lang": "de"}, {"value": "Abiotic depletion potential for non fossil resources (ADPE)", "lang": "en"}], "type": "LCIA method data set", "refObjectId": "b2ad6494-c78d-11e6-9d9d-cec0c932ce01", "uri": "../lciamethods/b2ad6494-c78d-11e6-9d9d-cec0c932ce01.xml"}, "other": {"anies": [{"name": "referenceToUnitGroupDataSet", "value": {"shortDescription": [{"value": "kg Sb-Äq.", "lang": "de"}], "type": "unit group data set", "refObjectId": "54ccd2d9-a32a-4fc2-923d-f2c8c93e89d4", "uri": "../unitgroups/54ccd2d9-a32a-4fc2-923d-f2c8c93e89d4.xml"}}, {"value": "0.000125", "module": "A1-A3"}, {"value": "9.58E-10", "module": "A5"}, {"value": "1.31E-10", "module": "C1"}, {"value": "8.99E-09", "module": "C2"}, {"value": "1.71E-08", "module": "C3"}, {"value": "1.25E-08", "module": "C4"}, {"value": "2.27E-05", "module": "D"}]}}, {"referenceToLCIAMethodDataSet": {"shortDescription": [{"value": "Potenzial für den abiotischen Abbau fossiler Brennstoffe (ADPF)", "lang": "de"}, {"value": "Abiotic depletion potential for fossil resources (ADPF)", "lang": "en"}], "type": "LCIA method data set", "refObjectId": "b2ad6110-c78d-11e6-9d9d-cec0c932ce01", "uri": "../lciamethods/b2ad6110-c78d-11e6-9d9d-cec0c932ce01.xml"}, "other": {"anies": [{"name": "referenceToUnitGroupDataSet", "value": {"shortDescription": [{"value": "MJ", "lang": "de"}], "type": "unit group data set", "refObjectId": "93a60a57-a3c8-11da-a746-0800200c9a66", "uri": "../unitgroups/93a60a57-a3c8-11da-a746-0800200c9a66.xml"}}, {"value": "359", "module": "A1-A3"}, {"value": "0.12", "module": "A5"}, {"value": "0.0234", "module": "C1"}, {"value": "1.17", "module": "C2"}, {"value": "1.44", "module": "C3"}, {"value": "1.6", "module": "C4"}, {"value": "-70.8", "module": "D"}]}}, {"referenceToLCIAMethodDataSet": {"shortDescription": [{"value": "Wassernutzung (WDP)", "lang": "de"}, {"value": "Water use (WDP)", "lang": "en"}], "type": "LCIA method data set", "refObjectId": "b2ad66ce-c78d-11e6-9d9d-cec0c932ce01", "uri": "../lciamethods/b2ad66ce-c78d-11e6-9d9d-cec0c932ce01.xml"}, "other": {"anies": [{"name": "referenceToUnitGroupDataSet", "value": {"shortDescription": [{"value": "m^(3) Welt-Äq. entzogen", "lang": "de"}], "type": "unit group data set", "refObjectId": "6ae2df01-888e-46c8-b17d-49fa3869b476", "uri": "../unitgroups/6ae2df01-888e-46c8-b17d-49fa3869b476.xml"}}, {"value": "2.92", "module": "A1-A3"}, {"value": "0.0402", "module": "A5"}, {"value": "8.24E-05", "module": "C1"}, {"value": "0.000995", "module": "C2"}, {"value": "0.305", "module": "C3"}, {"value": "0.0134", "module": "C4"}, {"value": "-0.739", "module": "D"}]}}, {"referenceToLCIAMethodDataSet": {"shortDescription": [{"value": "Auftreten von Krankheiten aufgrund von Feinstaubemissionen (PM)", "lang": "de"}, {"value": "Incidence of disease due to PM emissions (PM)", "lang": "en"}], "type": "LCIA method data set", "refObjectId": "b5c602c6-def3-11e6-bf01-fe55135034f3", "uri": "../lciamethods/b5c602c6-def3-11e6-bf01-fe55135034f3.xml"}, "other": {"anies": [{"name": "referenceToUnitGroupDataSet", "value": {"shortDescription": [{"value": "Krankheitsfälle", "lang": "de"}], "type": "unit group data set", "refObjectId": "3883559b-648f-4afc-8ba2-0bd24f3affa3", "uri": "../unitgroups/3883559b-648f-4afc-8ba2-0bd24f3affa3.xml"}}, {"value": "1.51E-06", "module": "A1-A3"}, {"value": "3.14E-10", "module": "A5"}, {"value": "1.45E-11", "module": "C1"}, {"value": "1.83E-09", "module": "C2"}, {"value": "4.23E-09", "module": "C3"}, {"value": "1.07E-08", "module": "C4"}, {"value": "-1.8E-07", "module": "D"}]}}, {"referenceToLCIAMethodDataSet": {"shortDescription": [{"value": "Wirkung durch Exposition des Menschen mit U235 (IR)", "lang": "de"}, {"value": "Human exposure efficiency relative to U235 (IR)", "lang": "en"}], "type": "LCIA method data set", "refObjectId": "b5c632be-def3-11e6-bf01-fe55135034f3", "uri": "../lciamethods/b5c632be-def3-11e6-bf01-fe55135034f3.xml"}, "other": {"anies": [{"name": "referenceToUnitGroupDataSet", "value": {"shortDescription": [{"value": "kBq U235-Äq.", "lang": "de"}], "type": "unit group data set", "refObjectId": "456b05bf-1415-44a9-9993-02452f554c09", "uri": "../unitgroups/456b05bf-1415-44a9-9993-02452f554c09.xml"}}, {"value": "2.17", "module": "A1-A3"}, {"value": "0.0013", "module": "A5"}, {"value": "0.00057", "module": "C1"}, {"value": "0.000329", "module": "C2"}, {"value": "0.0263", "module": "C3"}, {"value": "0.00198", "module": "C4"}, {"value": "-0.975", "module": "D"}]}}, {"referenceToLCIAMethodDataSet": {"shortDescription": [{"value": "Toxizitätsvergleichseinheit für Ökosysteme (ETP-fw)", "lang": "de"}, {"value": "Comparative toxic unit for ecosystems (ETP-fw)", "lang": "en"}], "type": "LCIA method data set", "refObjectId": "ee1082d1-b0f7-43ca-a1f0-21e2a4a74511", "uri": "../lciamethods/ee1082d1-b0f7-43ca-a1f0-21e2a4a74511.xml"}, "other": {"anies": [{"name": "referenceToUnitGroupDataSet", "value": {"shortDescription": [{"value": "CTUe", "lang": "de"}], "type": "unit group data set", "refObjectId": "aa959ded-f1eb-4efb-9c5c-2d60be36b3e6", "uri": "../unitgroups/aa959ded-f1eb-4efb-9c5c-2d60be36b3e6.xml"}}, {"value": "135", "module": "A1-A3"}, {"value": "0.0556", "module": "A5"}, {"value": "0.00717", "module": "C1"}, {"value": "0.83", "module": "C2"}, {"value": "0.593", "module": "C3"}, {"value": "0.898", "module": "C4"}, {"value": "-24.8", "module": "D"}]}}, {"referenceToLCIAMethodDataSet": {"shortDescription": [{"value": "Toxizitätsvergleichseinheit für Menschen (krebserregend) (HTP-c)", "lang": "de"}, {"value": "Comparative toxic unit for humans (carcinogenic) (HTP-c)", "lang": "en"}], "type": "LCIA method data set", "refObjectId": "2299222a-bbd8-474f-9d4f-4dd1f18aea7c", "uri": "../lciamethods/2299222a-bbd8-474f-9d4f-4dd1f18aea7c.xml"}, "other": {"anies": [{"name": "referenceToUnitGroupDataSet", "value": {"shortDescription": [{"value": "CTUh", "lang": "de"}], "type": "unit group data set", "refObjectId": "d4c9523e-2d7e-49fd-8469-998f547d3a70", "uri": "../unitgroups/d4c9523e-2d7e-49fd-8469-998f547d3a70.xml"}}, {"value": "6.6E-08", "module": "A1-A3"}, {"value": "2.92E-12", "module": "A5"}, {"value": "1.32E-13", "module": "C1"}, {"value": "1.71E-11", "module": "C2"}, {"value": "2.87E-11", "module": "C3"}, {"value": "1.37E-10", "module": "C4"}, {"value": "-3.56E-09", "module": "D"}]}}, {"referenceToLCIAMethodDataSet": {"shortDescription": [{"value": "Toxizitätsvergleichseinheit für Menschen (nicht krebserregend) (HTP-nc)", "lang": "de"}, {"value": "Comparative toxic unit for humans (noncarcinogenic) (HTP-nc)", "lang": "en"}], "type": "LCIA method data set", "refObjectId": "3af763a5-b7a1-48c9-9cee-1f223481fcef", "uri": "../lciamethods/3af763a5-b7a1-48c9-9cee-1f223481fcef.xml"}, "other": {"anies": [{"name": "referenceToUnitGroupDataSet", "value": {"shortDescription": [{"value": "CTUh", "lang": "de"}], "type": "unit group data set", "refObjectId": "d4c9523e-2d7e-49fd-8469-998f547d3a70", "uri": "../unitgroups/d4c9523e-2d7e-49fd-8469-998f547d3a70.xml"}}, {"value": "4.3E-07", "module": "A1-A3"}, {"value": "1.11E-10", "module": "A5"}, {"value": "6.71E-12", "module": "C1"}, {"value": "1.07E-09", "module": "C2"}, {"value": "1.03E-09", "module": "C3"}, {"value": "1.52E-08", "module": "C4"}, {"value": "-6.46E-08", "module": "D"}]}}, {"referenceToLCIAMethodDataSet": {"shortDescription": [{"value": "Bodenqualitätsindex (SQP)", "lang": "de"}, {"value": "Soil quality index (SQP)", "lang": "en"}], "type": "LCIA method data set", "refObjectId": "b2ad6890-c78d-11e6-9d9d-cec0c932ce01", "uri": "../lciamethods/b2ad6890-c78d-11e6-9d9d-cec0c932ce01.xml"}, "other": {"anies": [{"name": "referenceToUnitGroupDataSet", "value": {"shortDescription": [{"value": "SQP", "lang": "de"}], "type": "unit group data set", "refObjectId": "f130951c-e67f-4f7f-8dd4-665de3974e18", "uri": "../unitgroups/f130951c-e67f-4f7f-8dd4-665de3974e18.xml"}}, {"value": "127", "module": "A1-A3"}, {"value": "0.0335", "module": "A5"}, {"value": "0.00215", "module": "C1"}, {"value": "0.496", "module": "C2"}, {"value": "0.443", "module": "C3"}, {"value": "0.333", "module": "C4"}, {"value": "-4.99", "module": "D"}]}}]}, "otherAttributes": {"{http://www.indata.network/EPD/2019}epd-version": "1.2"}, "version": "1.1", "locations": "../ILCDLocations.xml"}