{"processInformation": {"dataSetInformation": {"UUID": "74afac2a-1d48-4246-bf20-1174260e683c", "name": {"baseName": [{"value": "MAGNA3 65-150 (Cast Iron)", "lang": "en"}, {"value": "MAGNA 3 65-150 (Gusseisen)", "lang": "de"}], "functionalUnitFlowProperties": [{"lang": "en"}]}, "classificationInformation": {"classification": [{"class": [{"value": "Gebäudetechnik", "level": 0, "classId": "8"}, {"value": "Heizung", "level": 1, "classId": "8.1"}, {"value": "Wärmeverteilung und Abgabe", "level": 2, "classId": "8.1.02"}], "name": "OEKOBAU.DAT"}, {"class": [{"value": "03 Building services engineering", "level": 0}, {"value": "Sanitary facilitys", "level": 1}, {"value": "Pumps for liquids and liquids with solids", "level": 2}], "name": "IBUCategories"}]}, "generalComment": [{"value": "The Grundfos MAGNA3 circulator pumps are designed for circulating liquids in heating systems, air conditioning and cooling systems and domestic hot water systems. However, the pump range can also be used in ground source heat pump systems and solar heating systems.\n\n\nThe MAGNA3 pump is a centrifugal pump powered by an electrical motor. It has a high-performance neodymium magnet rotor which increases motor efficiency and an insulation shell to reduce heat loss from the cast iron pump housing with threaded connections.\n\n\nThe declaration covers MAGNA3 65-150 pump.", "lang": "en"}, {"value": "Die Grundfos MAGNA3 Umwälzpumpen sind für die Umwälzung von Flüssigkeiten in Heizungsanlagen, Klima- und Kühlsystemen und Brauchwarmwasseranlagen konzipiert. Die Pumpenreihe kann jedoch auch in Erdwärmepumpensystemen und Solaranlagen eingesetzt werden. Die MAGNA3 Pumpe ist eine Kreiselpumpe, die von einem Elektromotor angetrieben wird. Sie verfügt über einen leistungsstarken Neodym-Magnetrotor, der den Wirkungsgrad des Motors erhöht, und eine Isolierschale, die den Wärmeverlust des gusseisernen Pumpengehäuses mit Gewindeanschlüssen verringert. Die Deklaration umfasst die MAGNA3 65-150 Pumpe.", "lang": "de"}]}, "quantitativeReference": {"referenceToReferenceFlow": [0]}, "time": {"referenceYear": 2023, "dataSetValidUntil": 2028, "other": {"anies": [{"name": "publicationDateOfEPD", "value": 1693440000000}]}}, "geography": {"locationOfOperationSupplyOrProduction": {"location": "DE"}}, "technology": {"technologyDescriptionAndIncludedProcesses": [{"value": "The Grundfos MAGNA3 circulation pumps are designed for circulating liquids in heating systems, air conditioning and cooling systems and domestic hot water systems. However, the pump series can also be used in geothermal heat pump systems and solar systems. \nTechnical data: \nThe performance data of the product according to the harmonized norms, based on the harmonization provisions above apply.\n\nThe relevant technical specifications according to the PCR Part B are given in the table below. \nDeclared unit: \nThe declared unit is 1 piece (pcs.) of MAGNA3 (Cast Iron) pump.", "lang": "en"}, {"value": "Die Grundfos MAGNA3 Umwälzpumpen sind für die Umwälzung von Flüssigkeiten in Heizungsanlagen, Klima- und Kühlsystemen und Brauchwarmwasseranlagen konzipiert. Die Pumpenreihe kann jedoch auch in Erdwärmepumpensystemen und Solaranlagen eingesetzt werden.  \nTechnische Daten: \nEs gelten die Leistungsdaten des Produkts gemäß den harmonisierten Normen, die auf den oben genannten Harmonisierungsbestimmungen basieren. Die relevanten technischen Spezifikationen gemäß PCR Teil B sind in der nachstehenden Tabelle aufgeführt. \nDeklarierte Einheit: \nBei der angegebenen Einheit handelt es sich um 1 Stück (Stk.) der MAGNA3 (Gusseisen) Pumpe.", "lang": "de"}], "technologicalApplicability": [{"value": "For the application and use the respective national provisions apply.\n\n\nThe pump is designed for circulating liquids in the\n\nfollowing systems:\n\n· heating systems\n\n· domestic hot-water systems\n\n· air-conditioning and cooling systems\n\n· ground-source heat-pump systems\n\n· solar-heating systems\n\nThe pump is suitable for thin, clean, non-aggressive and non-explosive liquids, not containing solid particles or fibres that may attack the pump mechanically or chemically. In heating systems, the water must meet the requirements of accepted standards on water quality in heating systems. The pumps are also suitable for domestic hot-water systems.", "lang": "en"}, {"value": "Für die Anwendung und den Einsatz gelten die jeweiligen nationalen Bestimmungen. Die Pumpe ist für die Umwälzung von Flüssigkeiten in folgenden Systemen ausgelegt: - Heizungsanlagen - Brauchwasseranlagen - Klima- und Kühlanlagen - Erdwärmepumpenanlagen - Solaranlagen Die Pumpe ist für dünne, saubere, nicht aggressive und nicht explosive Flüssigkeiten geeignet, die keine festen Partikel oder Fasern enthalten, die die Pumpe mechanisch oder chemisch angreifen könnten. In Heizungsanlagen muss das Wasser die Anforderungen der anerkannten Normen für die Wasserqualität in Heizungsanlagen erfüllen. Die Pumpen sind auch für Brauchwassersysteme geeignet.", "lang": "de"}]}}, "modellingAndValidation": {"LCIMethodAndAllocation": {"typeOfDataSet": "EPD", "referenceToLCAMethodDetails": [{"shortDescription": [{"value": "Pumps for liquids and liquids with solids.pdf", "lang": "en"}], "type": "source data set", "refObjectId": "38b7b7d2-5af7-4099-aebc-186dd4c2d631"}], "other": {"anies": [{"name": "subType", "value": "specific dataset"}]}}, "dataSourcesTreatmentAndRepresentativeness": {"referenceToDataSource": [{"shortDescription": [{"value": "GaBi Database (all versions)", "lang": "en"}], "type": "source data set", "refObjectId": "28d74cc0-db8b-4d7e-bc44-5f6d56ce0c4a"}, {"shortDescription": [{"value": "GaBi database SP40 2020", "lang": "en"}], "type": "source data set", "refObjectId": "0115289e-52f0-4920-bc7e-57b1c96aec8d"}], "useAdviceForDataSet": [{"value": "Scope: \nThe declaration applies to 1 piece of MAGNA3 (Cast Iron) pump. \n\nThe product is produced in Wahlstedt, Germany, and the life cycle assessment is based on data collected at the production site. \n\nProduction has been modeled using annual production data from 2021. \n\nThe declaration covers MAGNA3 65-150 product. \nSystem boundary: \nThis EPD is Cradle-To-Grave. The system boundaries\n\nof the EPD follow the modular approach in EN 15804. By decision no. 20170712-n of the SVR, the modules B3, B4 and B5 are by default declared as \"MNR\" (module not relevant).\n\nThe product stage (A1-A3) comprises raw material extraction and processing, transport processes as well as the manufacturing process. The final production and assembly of the MAGNA3 pump takes place at a Grundfos manufacturing site in Germany. However, the full supply-chain leading to the finished product at the gate is rather complex and includes a large amount of raw materials, components and semi-finished parts which come from both external suppliers as well as other Grundfos production facilities.\n\nThe product stage is included in the study, and according to EN 15804 the system boundary with nature is set to include those processes that provide the material and energy inputs into the system and the following manufacturing, transport up to the factory gate as well as the processing any waste arising from those processes.\n\nWastes and losses are included in the modules where they occur according to the polluter pays principle and the modular approach of EN 15804.\n\n\nThe product includes:\n\n· A1 Extraction and processing of raw materials;\n\n· A1 Reuse of products or materials from a previous product system;\n\n· A1 Processing of secondary materials;\n\n· A1 Generation of electricity, steam and heat from primary energy resources, also including their extraction, refining and transport;\n\n· A1 Energy recovery and other recovery processes from secondary fuels;\n\n· A2 Transportation up to the factory gate and internal transport;\n\n· A3 Production of ancillary materials or pre products;\n\n· A3 Manufacturing of products and coproducts;\n\n· A3 Manufacturing of packaging;\n\n· A1-A3 processing up to the end-of-waste state or disposal of final residues.\n\nFor secondary material inputs, the system boundary to the previous system (providing the secondary material) is set where outputs reach the end-of-waste state. The recycling of secondary material into new raw materials is included in the system boundary of this study. Waste\n\nmaterials from production processes that are recycled without any modification of the materials inherent characteristics are modelled as closed-loop within A1-A3. This is done up to the input mass flow that was used during production.\n\n\nWaste for incineration arising in the product stage is accounted for in the module where the waste is produced. The environmental loads from the incineration process are declared in the module where it occurs and the electricity and heat which is produced from the incineration are considered as closed-loop within A1-A3, as described in PCR Part A, 5.5.1. The input of biogenic carbon from the production of packaging material is inventoried in A3. As required by PCR Part A, the corresponding end-of-life module of the packaging material, A5, is also declared and the emissions of biogenic carbon are inventoried.\n\n\nThe construction process stage (A4-A5) includes:\n\nA4:\n\n· Transportation from factory gate to distribution centre:\n\n· Consumption of electricity, thermal energy and water at distribution centre;\n\n· Transportation from distribution centre to construction site;\n\n· Wastage during distribution.\n\nA5:\n\n· Installation process;\n\n· Transport of packaging waste to treatment site;\n\n· Waste treatment of packaging.\n\nThe packaging material does not reach the end of waste state but is incinerated as waste.\nAccording to European statistics, the average R1 value of incineration plants is > 0.6. Therefore, it is assumed\n\nthat packaging material is treated thermally in an incineration plant with R1 > 0.6. The loads from the combustion process of packaging are declared in module A5 and the resulting energy benefits in module\n\nD, as required by the PCR Part A, 5.5.2.\n\n\nUse stage (B1-B7):\n\n\nThe use stage, related to the building fabric includes:\n\n· B1, use or application of the installed product;\n\n· B2, maintenance.\n\nThe use stage related to the operation of the building\n\nincludes:\n\n· B6, operational energy use;\n\n· B7, operational water use.\n\nIn this study, all use stage modules are assessed, though B1, B2 and B7 are assessed to be zero. By decision no. 20170712-n of the SVR, the modules B3, B4 and B5 are by default declared as \"MNR\" (module\n\nnot relevant).\nThe modules include the provision and transport of all materials, products and related energy and water use, as well as waste processing up to the end-of-waste state or disposal of final residues during the use stage. They also include all impacts and\n\naspects related to the losses during the use stage (i.e. production, transport, and waste processing and disposal of the lost products and materials).\n\n\nGenerally, the geographical coverage of the datasets used matches the actual processes taking place. Meaning, that when modelling taking place in Grundfos Bjerringbro, the Danish electricity grid mix is used in the model and thermal energy from natural gas. These are generally of very high quality with very good technological, temporal and geographical representativeness.\n\n\nContributions to operational energy use during the use stage (B6) comes from the electricity consumption of the product. The annual electricity consumption is calculated by multiplying the average power input, which is based on a defined load profile, with the annual running hours. For use stage (B6) European Average electricity grid mix has been used. These values are declared in the scenarios section.\n\n\nThe End-of-Life stage (C1-C4) includes all activities from when the product reaches the end of its service life and no longer provides any functionality and until all materials and components are processed for\n\nreuse/recycling or disposed of.\n\n\nAccording to EN 15804 and the PCR Part A, the end-of-life stage includes:\n\n· C1 deconstruction of the product from the\n\n· building, including initial on-site sorting of the\n\n· materials;\n\n· C2 transportation of the discarded product to a recycling site and transportation of waste to final disposal;\n\n· C3 waste processing, collection of waste fractions from the deconstruction and waste processing of material flows intended for reuse, recycling and energy recovery;\n\n· C4 waste disposal including physical pretreatment and management of the disposal site.\n\nAt the end of life, the MAGNA3 pump is manually disassembled from the piping system in which it has been installed. The definition of the applied end-of-life scenario in this EPD follows the requirements in the\n\nPCR Part A, 6.2 regarding complex products, with a combination of recycling, thermal waste treatment and landfilling. 100 % of the material is considered in the end of life scenario as required by the PCR. An overall collection rate of 90 % has been assumed.\n\n\nMaterials from which energy is recovered in an incineration process with an R1-value above 0.60 are in this study included with the environmental burdens from the incineration process inventoried in C3, the recovered energy is declared as exported energy in C3\n\nand the energy benefits are declared in D. This procedure is according to the PCR Part A, 5.5.6. C3 includes the mechanical separation of the product followed by a series of sorting steps. Metal fractions are recycled and plastics, cardboard and electronics are assumed incinerated with energy recovery. The residual fractions are landfilled and declared in C4.\n\nThe specific amounts are shown in the scenarios section.\n\n\nBeyond system boundary (D): According to EN 15804 module D includes the reuse, recovery and/or recycling potentials, expressed as net impacts and benefits. Any declared benefits and loads from net\n\nflows leaving the product system that have not been allocated as co-products and that have passed the end-of-waste state are included in module D.\n\n\nContributions to module D comes from waste incineration processes in A5 and C3 as well as material recycling in C3. The specific fractions and net flows are shown in the scenarios section.", "lang": "en"}, {"value": "Gültigkeitsbereich: \nDie Deklaration bezieht sich auf 1 Stück der MAGNA3 (Gusseisen) Pumpe. \n\nDas Produkt wird in Wahlstedt, Deutschland, hergestellt. Die Ökobilanz basiert auf Daten, die am Produktionsstandort erhoben wurden. \n\nDie Produktion wurde anhand der jährlichen Produktionsdaten aus dem Jahr 2021 modelliert. \n\nDie Erklärung bezieht sich auf das Produkt MAGNA3 65-150. \nSystemgrenze: \nDiese EPD ist Cradle-To-Grave. Die Systemgrenzen der EPD folgen dem modularen Ansatz der EN 15804. Durch den Beschluss Nr. 20170712-n des SVR werden die Module B3, B4 und B5 standardmäßig als \"MNR\" (Modul nicht relevant) deklariert. Die Produktstufe (A1-A3) umfasst die Rohstoffgewinnung und -verarbeitung, Transportprozesse sowie den Herstellungsprozess. Die Endfertigung und Montage der MAGNA3-Pumpe findet in einer Grundfos-Produktionsstätte in Deutschland statt. Die gesamte Lieferkette, die zum fertigen Produkt an der Pforte führt, ist jedoch ziemlich komplex und umfasst eine große Menge an Rohstoffen, Komponenten und Halbfertigteilen, die sowohl von externen Lieferanten als auch von anderen Grundfos Produktionsstätten stammen.\n\nDie Produktphase wird in die Studie einbezogen, und gemäß EN 15804 wird die Systemgrenze mit der Natur so festgelegt, dass sie die Prozesse einschließt, die die Material- und Energiezufuhr in das System und die anschließende Herstellung, den Transport bis zum Werkstor sowie die Verarbeitung aller bei diesen Prozessen anfallenden Abfälle gewährleisten. Abfälle und Verluste werden gemäß dem Verursacherprinzip und dem modularen Ansatz der EN 15804 in den Modulen berücksichtigt, in denen sie auftreten.\n\n\nDas Produkt umfasst:\n\n- A1 Gewinnung und Verarbeitung von Rohstoffen; - A1 Wiederverwendung von Produkten oder Materialien aus einem früheren Produktsystem; - A1 Verarbeitung von Sekundärstoffen; - A1 Erzeugung von Strom, Dampf und Wärme aus Primärenergieressourcen, einschließlich deren Gewinnung, Raffination und Transport; - A1 Energierückgewinnung und andere Rückgewinnungsprozesse aus Sekundärbrennstoffen; - A2 Transport bis zum Werkstor und interner Transport; - A3 Herstellung von Hilfsstoffen oder Vorprodukten; - A3 Herstellung von Produkten und Koprodukten; - A3 Herstellung von Verpackungen; - A1-A3 Verarbeitung bis zum End-of-Waste-Zustand oder Entsorgung von Endresten.\n\nFür Sekundärmaterial-Inputs wird die Systemgrenze zum vorhergehenden System (das das Sekundärmaterial bereitstellt) dort festgelegt, wo die Outputs den Zustand am Ende der Abfallebene erreichen. Das Recycling von Sekundärmaterial zu neuen Rohstoffen ist in der Systemgrenze dieser Studie enthalten. Abfallstoffe aus Produktionsprozessen, die ohne Änderung der inhärenten Eigenschaften des Materials recycelt werden, werden als geschlossener Kreislauf innerhalb von A1-A3 modelliert. Dies geschieht bis zu dem Input-Massenstrom, der bei der Produktion verwendet wurde. Abfälle zur Verbrennung, die in der Produktphase anfallen, werden in dem Modul berücksichtigt, in dem der Abfall produziert wird. Die Umweltbelastungen aus dem Verbrennungsprozess werden in dem Modul angegeben, in dem er stattfindet, und der Strom und die Wärme, die bei der Verbrennung erzeugt werden, werden innerhalb von A1-A3 als geschlossener Kreislauf betrachtet, wie in PCR Teil A, 5.5.1 beschrieben. Der Eintrag von biogenem Kohlenstoff aus der Produktion von Verpackungsmaterial wird in A3 erfasst. Wie in PCR Teil A gefordert, wird auch das entsprechende End-of-Life-Modul des Verpackungsmaterials, A5, deklariert und die Emissionen von biogenem Kohlenstoff inventarisiert. Die Bauprozessphase (A4-A5) umfasst: A4: - Transport vom Werkstor zum Vertriebszentrum: - Verbrauch von Strom, Wärmeenergie und Wasser im Vertriebszentrum; - Transport vom Vertriebszentrum zur Baustelle; - Abfall während des Vertriebs.\n\nA5: - Installationsprozess; - Transport von Verpackungsabfällen zur Aufbereitungsanlage; - Abfallbehandlung von Verpackungen. Das Verpackungsmaterial erreicht nicht das Ende des Abfallstatus, sondern wird als Abfall verbrannt. Nach europäischen Statistiken liegt der durchschnittliche R1-Wert von Verbrennungsanlagen bei > 0,6. Daher wird davon ausgegangen, dass Verpackungsmaterial in einer Verbrennungsanlage mit R1 > 0,6 thermisch behandelt wird. Die Lasten aus dem Verbrennungsprozess von Verpackungen werden in Modul A5 angegeben und die daraus resultierenden Energievorteile in Modul D, wie in PCR Teil A, 5.5.2 gefordert. Nutzungsphase (B1-B7): Die Nutzungsphase, die sich auf die Bausubstanz bezieht, umfasst: - B1, Nutzung oder Anwendung des installierten Produkts; - B2, Instandhaltung. Die Nutzungsphase, die sich auf den Betrieb des Gebäudes bezieht, umfasst: - B6, betrieblicher Energieverbrauch; - B7, betrieblicher Wasserverbrauch. In dieser Studie werden alle Module der Nutzungsphase bewertet, wobei B1, B2 und B7 als Null bewertet werden. Durch den Beschluss Nr. 20170712-n des SVR werden die Module B3, B4 und B5 standardmäßig als \"MNR\" (Modul nicht relevant) deklariert. Die Module umfassen die Bereitstellung und den Transport aller Materialien, Produkte und den damit verbundenen Energie- und Wasserverbrauch sowie die Abfallverarbeitung bis zum End-of-Waste-Zustand oder die Entsorgung von Endresten während der Nutzungsphase. Sie umfassen auch alle Auswirkungen und Aspekte im Zusammenhang mit den Verlusten während der Nutzungsphase (d.h. Produktion, Transport, Abfallverarbeitung und Entsorgung der verlorenen Produkte und Materialien). Im Allgemeinen entspricht die geographische Abdeckung der verwendeten Datensätze den tatsächlich stattfindenden Prozessen. Das bedeutet, dass bei der Modellierung in Grundfos Bjerringbro der dänische Stromnetzmix im Modell verwendet wird und die Wärmeenergie aus Erdgas. Diese sind im Allgemeinen von sehr hoher Qualität mit sehr guter technologischer, zeitlicher und geografischer Repräsentativität. Der Beitrag zum betrieblichen Energieverbrauch während der Nutzungsphase (B6) stammt aus dem Stromverbrauch des Produkts. Der jährliche Stromverbrauch wird berechnet, indem die durchschnittliche Leistungsaufnahme, die auf einem definierten Lastprofil basiert, mit den jährlichen Betriebsstunden multipliziert wird. Für die Nutzungsphase (B6) wurde der durchschnittliche europäische Stromnetzmix verwendet. Diese Werte werden im Abschnitt Szenarien angegeben. Die End-of-Life-Phase (C1-C4) umfasst alle Aktivitäten ab dem Zeitpunkt, an dem das Produkt das Ende seiner Lebensdauer erreicht hat und keine Funktionalität mehr bietet und bis alle Materialien und Komponenten für die Wiederverwendung/Recycling aufbereitet oder entsorgt werden.\n\n\nGemäß EN 15804 und dem PCR Teil A umfasst die End-of-Life-Phase: - C1 Rückbau des Produkts aus dem - Gebäude, einschließlich einer ersten Sortierung der - Materialien vor Ort; - C2 Transport des ausrangierten Produkts zu einer Recyclinganlage und Transport der Abfälle zur endgültigen Entsorgung; - C3 Abfallverarbeitung, Sammlung von Abfallfraktionen aus dem Rückbau und Abfallverarbeitung von Stoffströmen, die für die Wiederverwendung, das Recycling und die Energierückgewinnung bestimmt sind; - C4 Abfallentsorgung, einschließlich physikalischer Vorbehandlung und Verwaltung der Deponie.\n\nAm Ende der Lebensdauer wird die MAGNA3-Pumpe manuell aus dem Rohrleitungssystem, in das sie eingebaut wurde, demontiert. Die Definition des angewandten End-of-Life-Szenarios in dieser EPD folgt den Anforderungen des PCR Teil A, 6.2 in Bezug auf komplexe Produkte, mit einer Kombination aus Recycling, thermischer Abfallbehandlung und Deponierung. 100 % des Materials werden im End-of-Life-Szenario berücksichtigt, wie in der PCR gefordert. Es wurde eine Gesamtsammelquote von 90 % angenommen. Materialien, aus denen in einem Verbrennungsprozess mit einem R1-Wert von über 0,60 Energie zurückgewonnen wird, werden in dieser Studie mit den Umweltbelastungen aus dem Verbrennungsprozess in C3 erfasst, die zurückgewonnene Energie wird als exportierte Energie in C3 angegeben und die Energievorteile werden in D angegeben. Dieses Verfahren entspricht dem PCR Teil A, 5.5.6. C3 umfasst die mechanische Trennung des Produkts, gefolgt von einer Reihe von Sortierschritten. Die Metallfraktionen werden recycelt und es wird angenommen, dass Kunststoffe, Karton und Elektronik mit Energierückgewinnung verbrannt werden. Die verbleibenden Fraktionen werden deponiert und in C4 deklariert. Die spezifischen Mengen sind im Abschnitt Szenarien aufgeführt. Jenseits der Systemgrenze (D): Gemäß EN 15804 umfasst Modul D die Wiederverwendungs-, Verwertungs- und/oder Recyclingpotenziale, ausgedrückt als Nettoauswirkungen und Nutzen. Alle deklarierten Vorteile und Belastungen aus Nettoströmen, die das Produktsystem verlassen, die nicht als Nebenprodukte zugeordnet wurden und die das Abfallende überschritten haben, sind in Modul D enthalten. Beiträge zu Modul D stammen aus den Abfallverbrennungsprozessen in A5 und C3 sowie aus dem Materialrecycling in C3. Die spezifischen Fraktionen und Nettoströme sind im Abschnitt Szenarien aufgeführt.", "lang": "de"}], "other": {"anies": [{"name": "referenceToOriginalEPD", "value": {"shortDescription": {"value": "MAGNA3 65-150 (Cast Iron).pdf", "defaultValue": "MAGNA3 65-150 (Cast Iron).pdf", "lstrings": [{"lang": "en", "value": "MAGNA3 65-150 (Cast Iron).pdf"}]}, "type": "source data set", "uuid": {"uuid": "87bb4ec9-408e-4195-bc59-7d3f5b0fffe2"}, "refObjectId": "87bb4ec9-408e-4195-bc59-7d3f5b0fffe2", "resourceURLs": ["https://oekobaudat.de/OEKOBAU.DAT/resource/sources/87bb4ec9-408e-4195-bc59-7d3f5b0fffe2/MAGNA3_65-150_Cast_Iron__19088.pdf?version=00.02.000"]}}]}}, "validation": {"review": [{"referenceToNameOfReviewerAndInstitution": [{"shortDescription": [{"value": "Institut Bauen und Umwelt e. V.", "lang": "en"}], "type": "contact data set", "refObjectId": "d111dbec-b024-4be5-86c5-752d6eb2cf95", "uri": "../contacts/d111dbec-b024-4be5-86c5-752d6eb2cf95.xml"}], "type": "Accredited third party review"}]}, "complianceDeclarations": {"compliance": [{"referenceToComplianceSystem": {"shortDescription": [{"value": "DIN EN 15804+A2", "lang": "en"}], "type": "source data set", "refObjectId": "c0016b33-8cf7-415c-ac6e-deba0d21440d", "uri": "../sources/c0016b33-8cf7-415c-ac6e-deba0d21440d.xml"}}, {"referenceToComplianceSystem": {"shortDescription": [{"value": "ISO 14025", "lang": "en"}], "type": "source data set", "refObjectId": "4f2eb655-6e44-4874-a95a-e28f5442cd4d", "uri": "../sources/4f2eb655-6e44-4874-a95a-e28f5442cd4d.xml"}}]}}, "administrativeInformation": {"commissionerAndGoal": {"referenceToCommissioner": [{"shortDescription": [{"value": "Grundfos Holding A/S", "lang": "en"}], "type": "contact data set", "refObjectId": "de0c5e18-bdc1-43d3-bfd4-abb2d5105bed", "uri": "../contacts/de0c5e18-bdc1-43d3-bfd4-abb2d5105bed.xml"}]}, "dataGenerator": {"referenceToPersonOrEntityGeneratingTheDataSet": [{"shortDescription": [{"value": "Grundfos Holding A/S", "lang": "en"}], "type": "contact data set", "refObjectId": "de0c5e18-bdc1-43d3-bfd4-abb2d5105bed", "uri": "../contacts/de0c5e18-bdc1-43d3-bfd4-abb2d5105bed.xml"}]}, "dataEntryBy": {"timeStamp": 1693440000000, "referenceToDataSetFormat": [{"shortDescription": [{"value": "ILCD Format", "lang": "en"}], "type": "source data set", "refObjectId": "a97a0155-0234-4b87-b4ce-a45da52f2a40", "uri": "../sources/a97a0155-0234-4b87-b4ce-a45da52f2a40.xml"}, {"shortDescription": [{"value": "EPD-Datenformaterweiterungen v1.2", "lang": "de"}, {"value": "EPD Data Format Extensions v1.2", "lang": "en"}], "type": "source data set", "refObjectId": "a29449fd-aa2f-4de8-b5d7-4b06b43c6fde", "uri": "../sources/a29449fd-aa2f-4de8-b5d7-4b06b43c6fde.xml"}]}, "publicationAndOwnership": {"dataSetVersion": "00.08.000", "referenceToRegistrationAuthority": {"shortDescription": [{"value": "Institut Bauen und Umwelt e. V.", "lang": "en"}], "type": "contact data set", "refObjectId": "d111dbec-b024-4be5-86c5-752d6eb2cf95", "uri": "../contacts/d111dbec-b024-4be5-86c5-752d6eb2cf95.xml"}, "registrationNumber": "EPD-GRU-20230069-CBC2-EN", "referenceToOwnershipOfDataSet": {"shortDescription": [{"value": "Grundfos Holding A/S", "lang": "en"}], "type": "contact data set", "refObjectId": "de0c5e18-bdc1-43d3-bfd4-abb2d5105bed", "uri": "../contacts/de0c5e18-bdc1-43d3-bfd4-abb2d5105bed.xml"}, "copyright": true, "licenseType": "Free of charge for all users and uses", "accessRestrictions": [{"value": "None", "lang": "en"}], "other": {"anies": [{"name": "referenceToPublisher", "value": {"shortDescription": [{"value": "Institut Bauen und Umwelt e. V.", "lang": "en"}], "type": "contact data set", "refObjectId": "d111dbec-b024-4be5-86c5-752d6eb2cf95", "uri": "../contacts/d111dbec-b024-4be5-86c5-752d6eb2cf95.xml"}}]}}}, "exchanges": {"exchange": [{"dataSetInternalID": 0, "referenceToFlowDataSet": {"shortDescription": [{"value": " MAGNA3 65-150 (Cast Iron) (MAGNA 3 65-150 (Gusseisen))", "lang": "en"}], "type": "flow data set", "refObjectId": "d9c01d50-d896-d78b-8817-71b27f537f2a", "uri": "../flows/d9c01d50-d896-d78b-8817-71b27f537f2a.xml"}, "meanAmount": 1.0, "referencesToDataSource": {}, "referenceFlow": true, "resolvedFlowVersion": "00.02.000", "resultingflowAmount": 1.0, "flowProperties": [{"name": [{"lang": "de", "value": "Anzahl"}, {"lang": "en", "value": "Number of pieces"}], "uuid": "01846770-4cfe-4a25-8ad9-919d8d378345", "referenceFlowProperty": true, "meanValue": 1.0, "referenceUnit": "pcs.", "unitGroupUUID": "934110e3-baf4-49e9-992c-3d8109a6aafb"}], "materialProperties": [{"name": "weight per piece", "value": "26.3", "unit": "kg"}], "typeOfFlow": "Product flow", "classification": {"classHierarchy": "Metalle / Stahl und Eisen / ", "name": "OEKOBAU.DAT"}}, {"dataSetInternalID": 1, "referenceToFlowDataSet": {"shortDescription": [{"value": "Renewable primary energy as energy carrier (PERE)", "lang": "en"}, {"value": "Erneuerbare Primärenergie als Energieträger (PERE)", "lang": "de"}], "type": "flow data set", "refObjectId": "20f32be5-0398-4288-9b6d-accddd195317", "uri": "../flows/20f32be5-0398-4288-9b6d-accddd195317.xml"}, "exchange direction": "INPUT", "other": {"anies": [{"name": "referenceToUnitGroupDataSet", "value": {"shortDescription": [{"value": "MJ", "lang": "en"}], "type": "unit group data set", "refObjectId": "93a60a57-a3c8-11da-a746-0800200c9a66", "uri": "../unitgroups/93a60a57-a3c8-11da-a746-0800200c9a66.xml"}}, {"value": "405.0632462", "module": "A1"}, {"value": "1.087726129", "module": "A2"}, {"value": "51.23028388", "module": "A3"}, {"value": "1.362293099", "module": "A4"}, {"value": "0.169781621", "module": "A5"}, {"value": "8814.019978", "module": "B6"}, {"value": "0", "module": "C1"}, {"value": "0.521026536", "module": "C2"}, {"value": "19.26106852", "module": "C3"}, {"value": "0.162622601", "module": "C4"}, {"value": "7.860333071", "module": "D"}]}, "resolvedFlowVersion": "38.00.000", "flowProperties": [], "typeOfFlow": "Other flow", "classification": {"classHierarchy": "Quantities", "name": "GaBiCategories"}}, {"dataSetInternalID": 2, "referenceToFlowDataSet": {"shortDescription": [{"value": "Renewable primary energy resources as material utilization (PERM)", "lang": "en"}, {"value": "Erneuerbare Primärenergie zur stofflichen Nutzung (PERM)", "lang": "de"}], "type": "flow data set", "refObjectId": "fb3ec0de-548d-4508-aea5-00b73bf6f702", "uri": "../flows/fb3ec0de-548d-4508-aea5-00b73bf6f702.xml"}, "exchange direction": "INPUT", "other": {"anies": [{"name": "referenceToUnitGroupDataSet", "value": {"shortDescription": [{"value": "MJ", "lang": "en"}], "type": "unit group data set", "refObjectId": "93a60a57-a3c8-11da-a746-0800200c9a66", "uri": "../unitgroups/93a60a57-a3c8-11da-a746-0800200c9a66.xml"}}, {"value": "0", "module": "A1"}, {"value": "0", "module": "A2"}, {"value": "0", "module": "A3"}, {"value": "0", "module": "A4"}, {"value": "0", "module": "A5"}, {"value": "0", "module": "B6"}, {"value": "0", "module": "C1"}, {"value": "0", "module": "C2"}, {"value": "0", "module": "C3"}, {"value": "0", "module": "C4"}, {"value": "0", "module": "D"}]}, "resolvedFlowVersion": "38.00.000", "flowProperties": [], "typeOfFlow": "Other flow", "classification": {"classHierarchy": "Quantities", "name": "GaBiCategories"}}, {"dataSetInternalID": 3, "referenceToFlowDataSet": {"shortDescription": [{"value": "Total use of renewable primary energy resources (PERT)", "lang": "en"}, {"value": "Total erneuerbare Primärenergie (PERT)", "lang": "de"}], "type": "flow data set", "refObjectId": "53f97275-fa8a-4cdd-9024-65936002acd0", "uri": "../flows/53f97275-fa8a-4cdd-9024-65936002acd0.xml"}, "exchange direction": "INPUT", "other": {"anies": [{"name": "referenceToUnitGroupDataSet", "value": {"shortDescription": [{"value": "MJ", "lang": "en"}], "type": "unit group data set", "refObjectId": "93a60a57-a3c8-11da-a746-0800200c9a66", "uri": "../unitgroups/93a60a57-a3c8-11da-a746-0800200c9a66.xml"}}, {"value": "405.0632462", "module": "A1"}, {"value": "1.087726129", "module": "A2"}, {"value": "51.23028388", "module": "A3"}, {"value": "1.362293099", "module": "A4"}, {"value": "0.169781621", "module": "A5"}, {"value": "8814.019978", "module": "B6"}, {"value": "0", "module": "C1"}, {"value": "0.521026536", "module": "C2"}, {"value": "19.26106852", "module": "C3"}, {"value": "0.162622601", "module": "C4"}, {"value": "7.860333071", "module": "D"}]}, "resolvedFlowVersion": "38.00.000", "flowProperties": [], "typeOfFlow": "Other flow", "classification": {"classHierarchy": "Quantities / Environmental quantities / EPD EN 15804 / LCI indicators", "name": "GaBiCategories"}}, {"dataSetInternalID": 4, "referenceToFlowDataSet": {"shortDescription": [{"value": "Non renewable primary energy as energy carrier (PENRE)", "lang": "en"}, {"value": "Nicht-erneuerbare Primärenergie als Energieträger (PENRE)", "lang": "de"}], "type": "flow data set", "refObjectId": "ac857178-2b45-46ec-892a-a9a4332f0372", "uri": "../flows/ac857178-2b45-46ec-892a-a9a4332f0372.xml"}, "exchange direction": "INPUT", "other": {"anies": [{"name": "referenceToUnitGroupDataSet", "value": {"shortDescription": [{"value": "MJ", "lang": "en"}], "type": "unit group data set", "refObjectId": "93a60a57-a3c8-11da-a746-0800200c9a66", "uri": "../unitgroups/93a60a57-a3c8-11da-a746-0800200c9a66.xml"}}, {"value": "1492.230083", "module": "A1"}, {"value": "20.64884021", "module": "A2"}, {"value": "56.78032931", "module": "A3"}, {"value": "21.99287914", "module": "A4"}, {"value": "0.985882821", "module": "A5"}, {"value": "19889.50025", "module": "B6"}, {"value": "0", "module": "C1"}, {"value": "9.047211122", "module": "C2"}, {"value": "44.36224645", "module": "C3"}, {"value": "2.318022109", "module": "C4"}, {"value": "-26.62767751", "module": "D"}]}, "resolvedFlowVersion": "38.00.000", "flowProperties": [], "typeOfFlow": "Other flow", "classification": {"classHierarchy": "Quantities", "name": "GaBiCategories"}}, {"dataSetInternalID": 5, "referenceToFlowDataSet": {"shortDescription": [{"value": "Non renewable primary energy as material utilization (PENRM)", "lang": "en"}, {"value": "Nicht-erneuerbare Primärenergie zur stofflichen Nutzung (PENRM)", "lang": "de"}], "type": "flow data set", "refObjectId": "1421caa0-679d-4bf4-b282-0eb850ccae27", "uri": "../flows/1421caa0-679d-4bf4-b282-0eb850ccae27.xml"}, "exchange direction": "INPUT", "other": {"anies": [{"name": "referenceToUnitGroupDataSet", "value": {"shortDescription": [{"value": "MJ", "lang": "en"}], "type": "unit group data set", "refObjectId": "93a60a57-a3c8-11da-a746-0800200c9a66", "uri": "../unitgroups/93a60a57-a3c8-11da-a746-0800200c9a66.xml"}}, {"value": "0", "module": "A1"}, {"value": "0", "module": "A2"}, {"value": "0", "module": "A3"}, {"value": "0", "module": "A4"}, {"value": "0", "module": "A5"}, {"value": "0", "module": "B6"}, {"value": "0", "module": "C1"}, {"value": "0", "module": "C2"}, {"value": "0", "module": "C3"}, {"value": "0", "module": "C4"}, {"value": "0", "module": "D"}]}, "resolvedFlowVersion": "38.00.000", "flowProperties": [], "typeOfFlow": "Other flow", "classification": {"classHierarchy": "Quantities", "name": "GaBiCategories"}}, {"dataSetInternalID": 6, "referenceToFlowDataSet": {"shortDescription": [{"value": "Total use of non renewable primary energy resources (PENRT)", "lang": "en"}, {"value": "Total nicht erneuerbare Primärenergie (PENRT)", "lang": "de"}], "type": "flow data set", "refObjectId": "06159210-646b-4c8d-8583-da9b3b95a6c1", "uri": "../flows/06159210-646b-4c8d-8583-da9b3b95a6c1.xml"}, "exchange direction": "INPUT", "other": {"anies": [{"name": "referenceToUnitGroupDataSet", "value": {"shortDescription": [{"value": "MJ", "lang": "en"}], "type": "unit group data set", "refObjectId": "93a60a57-a3c8-11da-a746-0800200c9a66", "uri": "../unitgroups/93a60a57-a3c8-11da-a746-0800200c9a66.xml"}}, {"value": "1492.231017", "module": "A1"}, {"value": "20.64884021", "module": "A2"}, {"value": "56.78032931", "module": "A3"}, {"value": "21.99287933", "module": "A4"}, {"value": "0.985882821", "module": "A5"}, {"value": "19889.50025", "module": "B6"}, {"value": "0", "module": "C1"}, {"value": "9.047211122", "module": "C2"}, {"value": "44.36224645", "module": "C3"}, {"value": "2.318022109", "module": "C4"}, {"value": "-26.62767751", "module": "D"}]}, "resolvedFlowVersion": "38.00.000", "flowProperties": [], "typeOfFlow": "Other flow", "classification": {"classHierarchy": "Quantities / Environmental quantities / EPD EN 15804 / LCI indicators", "name": "GaBiCategories"}}, {"dataSetInternalID": 7, "referenceToFlowDataSet": {"shortDescription": [{"value": "Use of secondary material (SM)", "lang": "en"}, {"value": "Einsatz von Sekundärstoffen (SM)", "lang": "de"}], "type": "flow data set", "refObjectId": "c6a1f35f-2d09-4f54-8dfb-97e502e1ce92", "uri": "../flows/c6a1f35f-2d09-4f54-8dfb-97e502e1ce92.xml"}, "exchange direction": "INPUT", "other": {"anies": [{"name": "referenceToUnitGroupDataSet", "value": {"shortDescription": [{"value": "kg", "lang": "en"}], "type": "unit group data set", "refObjectId": "ad38d542-3fe9-439d-9b95-2f5f7752acaf", "uri": "../unitgroups/ad38d542-3fe9-439d-9b95-2f5f7752acaf.xml"}}, {"value": "19.2113451", "module": "A1"}, {"value": "0", "module": "A2"}, {"value": "0.240428894", "module": "A3"}, {"value": "0.003890355", "module": "A4"}, {"value": "0", "module": "A5"}, {"value": "0", "module": "B6"}, {"value": "0", "module": "C1"}, {"value": "0", "module": "C2"}, {"value": "0", "module": "C3"}, {"value": "0", "module": "C4"}, {"value": "0", "module": "D"}]}, "resolvedFlowVersion": "38.00.000", "flowProperties": [], "typeOfFlow": "Other flow", "classification": {"classHierarchy": "Quantities / Environmental quantities / EPD EN 15804 / LCI indicators", "name": "GaBiCategories"}}, {"dataSetInternalID": 8, "referenceToFlowDataSet": {"shortDescription": [{"value": "Use of renewable secondary fuels (RSF)", "lang": "en"}, {"value": "Erneuerbare Sekundärbrennstoffe (RSF)", "lang": "de"}], "type": "flow data set", "refObjectId": "64333088-a55f-4aa2-9a31-c10b07816787", "uri": "../flows/64333088-a55f-4aa2-9a31-c10b07816787.xml"}, "exchange direction": "INPUT", "other": {"anies": [{"name": "referenceToUnitGroupDataSet", "value": {"shortDescription": [{"value": "MJ", "lang": "en"}], "type": "unit group data set", "refObjectId": "93a60a57-a3c8-11da-a746-0800200c9a66", "uri": "../unitgroups/93a60a57-a3c8-11da-a746-0800200c9a66.xml"}}, {"value": "1.46E-23", "module": "A1"}, {"value": "0", "module": "A2"}, {"value": "0", "module": "A3"}, {"value": "2.91E-27", "module": "A4"}, {"value": "0", "module": "A5"}, {"value": "0", "module": "B6"}, {"value": "0", "module": "C1"}, {"value": "0", "module": "C2"}, {"value": "0", "module": "C3"}, {"value": "0", "module": "C4"}, {"value": "0", "module": "D"}]}, "resolvedFlowVersion": "38.00.000", "flowProperties": [], "typeOfFlow": "Other flow", "classification": {"classHierarchy": "Quantities / Environmental quantities / EPD EN 15804 / LCI indicators", "name": "GaBiCategories"}}, {"dataSetInternalID": 9, "referenceToFlowDataSet": {"shortDescription": [{"value": "Use of non renewable secondary fuels (NRSF)", "lang": "en"}, {"value": "Nicht erneuerbare Sekundärbrennstoffe (NRSF)", "lang": "de"}], "type": "flow data set", "refObjectId": "89def144-d39a-4287-b86f-efde453ddcb2", "uri": "../flows/89def144-d39a-4287-b86f-efde453ddcb2.xml"}, "exchange direction": "INPUT", "other": {"anies": [{"name": "referenceToUnitGroupDataSet", "value": {"shortDescription": [{"value": "MJ", "lang": "en"}], "type": "unit group data set", "refObjectId": "93a60a57-a3c8-11da-a746-0800200c9a66", "uri": "../unitgroups/93a60a57-a3c8-11da-a746-0800200c9a66.xml"}}, {"value": "1.71E-22", "module": "A1"}, {"value": "0", "module": "A2"}, {"value": "0", "module": "A3"}, {"value": "3.42E-26", "module": "A4"}, {"value": "0", "module": "A5"}, {"value": "0", "module": "B6"}, {"value": "0", "module": "C1"}, {"value": "0", "module": "C2"}, {"value": "0", "module": "C3"}, {"value": "0", "module": "C4"}, {"value": "0", "module": "D"}]}, "resolvedFlowVersion": "38.00.000", "flowProperties": [], "typeOfFlow": "Other flow", "classification": {"classHierarchy": "Quantities / Environmental quantities / EPD EN 15804 / LCI indicators", "name": "GaBiCategories"}}, {"dataSetInternalID": 10, "referenceToFlowDataSet": {"shortDescription": [{"value": "Use of net fresh water (FW)", "lang": "en"}, {"value": "Einsatz von Süßwasserressourcen (FW)", "lang": "de"}], "type": "flow data set", "refObjectId": "3cf952c8-f3a4-461d-8c96-96456ca62246", "uri": "../flows/3cf952c8-f3a4-461d-8c96-96456ca62246.xml"}, "exchange direction": "INPUT", "other": {"anies": [{"name": "referenceToUnitGroupDataSet", "value": {"shortDescription": [{"value": "m^3", "lang": "en"}], "type": "unit group data set", "refObjectId": "cd950537-0a98-4044-9ba7-9f9a68d0a504", "uri": "../unitgroups/cd950537-0a98-4044-9ba7-9f9a68d0a504.xml"}}, {"value": "0.84235956", "module": "A1"}, {"value": "0.00127156", "module": "A2"}, {"value": "0.026067828", "module": "A3"}, {"value": "0.001662875", "module": "A4"}, {"value": "0.008288171", "module": "A5"}, {"value": "10.19122507", "module": "B6"}, {"value": "0", "module": "C1"}, {"value": "0.000607171", "module": "C2"}, {"value": "0.032704547", "module": "C3"}, {"value": "2.95E-05", "module": "C4"}, {"value": "0.026360166", "module": "D"}]}, "resolvedFlowVersion": "38.00.000", "flowProperties": [], "typeOfFlow": "Other flow", "classification": {"classHierarchy": "Quantities / Environmental quantities / EPD EN 15804 / LCI indicators", "name": "GaBiCategories"}}, {"dataSetInternalID": 11, "referenceToFlowDataSet": {"shortDescription": [{"value": "Hazardous waste disposed (HWD)", "lang": "en"}, {"value": "Gefährlicher Abfall zur Deponie (HWD)", "lang": "de"}], "type": "flow data set", "refObjectId": "430f9e0f-59b2-46a0-8e0d-55e0e84948fc", "uri": "../flows/430f9e0f-59b2-46a0-8e0d-55e0e84948fc.xml"}, "exchange direction": "OUTPUT", "other": {"anies": [{"name": "referenceToUnitGroupDataSet", "value": {"shortDescription": [{"value": "kg", "lang": "en"}], "type": "unit group data set", "refObjectId": "ad38d542-3fe9-439d-9b95-2f5f7752acaf", "uri": "../unitgroups/ad38d542-3fe9-439d-9b95-2f5f7752acaf.xml"}}, {"value": "0.000330482", "module": "A1"}, {"value": "8.69E-07", "module": "A2"}, {"value": "0.000121779", "module": "A3"}, {"value": "1.07E-06", "module": "A4"}, {"value": "5.11E-09", "module": "A5"}, {"value": "8.23E-06", "module": "B6"}, {"value": "0", "module": "C1"}, {"value": "4.18E-07", "module": "C2"}, {"value": "2.2E-08", "module": "C3"}, {"value": "9.29E-09", "module": "C4"}, {"value": "-0.000328251", "module": "D"}]}, "resolvedFlowVersion": "38.00.000", "flowProperties": [], "typeOfFlow": "Other flow", "classification": {"classHierarchy": "Quantities / Environmental quantities / EPD EN 15804 / LCI indicators", "name": "GaBiCategories"}}, {"dataSetInternalID": 12, "referenceToFlowDataSet": {"shortDescription": [{"value": "Non hazardous waste disposed (NHWD)", "lang": "en"}, {"value": "Entsorgter nicht gefährlicher Abfall (NHWD)", "lang": "de"}], "type": "flow data set", "refObjectId": "b29ef66b-e286-4afa-949f-62f1a7b4d7fa", "uri": "../flows/b29ef66b-e286-4afa-949f-62f1a7b4d7fa.xml"}, "exchange direction": "OUTPUT", "other": {"anies": [{"name": "referenceToUnitGroupDataSet", "value": {"shortDescription": [{"value": "kg", "lang": "en"}], "type": "unit group data set", "refObjectId": "ad38d542-3fe9-439d-9b95-2f5f7752acaf", "uri": "../unitgroups/ad38d542-3fe9-439d-9b95-2f5f7752acaf.xml"}}, {"value": "5.167548462", "module": "A1"}, {"value": "0.003167996", "module": "A2"}, {"value": "0.295680241", "module": "A3"}, {"value": "0.004734404", "module": "A4"}, {"value": "0.094327585", "module": "A5"}, {"value": "14.1099998", "module": "B6"}, {"value": "0", "module": "C1"}, {"value": "0.001433913", "module": "C2"}, {"value": "0.690055633", "module": "C3"}, {"value": "2.654950828", "module": "C4"}, {"value": "2.125542196", "module": "D"}]}, "resolvedFlowVersion": "38.00.000", "flowProperties": [], "typeOfFlow": "Other flow", "classification": {"classHierarchy": "Quantities / Environmental quantities / EPD EN 15804 / LCI indicators", "name": "GaBiCategories"}}, {"dataSetInternalID": 13, "referenceToFlowDataSet": {"shortDescription": [{"value": "Radioactive waste disposed (RWD)", "lang": "en"}, {"value": "Entsorgter radioaktiver Abfall (RWD)", "lang": "de"}], "type": "flow data set", "refObjectId": "3449546e-52ad-4b39-b809-9fb77cea8ff6", "uri": "../flows/3449546e-52ad-4b39-b809-9fb77cea8ff6.xml"}, "exchange direction": "OUTPUT", "other": {"anies": [{"name": "referenceToUnitGroupDataSet", "value": {"shortDescription": [{"value": "kg", "lang": "en"}], "type": "unit group data set", "refObjectId": "ad38d542-3fe9-439d-9b95-2f5f7752acaf", "uri": "../unitgroups/ad38d542-3fe9-439d-9b95-2f5f7752acaf.xml"}}, {"value": "0.062533239", "module": "A1"}, {"value": "3.67E-05", "module": "A2"}, {"value": "0.001567925", "module": "A3"}, {"value": "5.79E-05", "module": "A4"}, {"value": "4.74E-05", "module": "A5"}, {"value": "3.01797548", "module": "B6"}, {"value": "0", "module": "C1"}, {"value": "1.67E-05", "module": "C2"}, {"value": "0.006578442", "module": "C3"}, {"value": "2.78E-05", "module": "C4"}, {"value": "-0.001060569", "module": "D"}]}, "resolvedFlowVersion": "38.00.000", "flowProperties": [], "typeOfFlow": "Other flow", "classification": {"classHierarchy": "Quantities / Environmental quantities / EPD EN 15804 / LCI indicators", "name": "GaBiCategories"}}, {"dataSetInternalID": 14, "referenceToFlowDataSet": {"shortDescription": [{"value": "Components for re-use (CRU)", "lang": "en"}, {"value": "Komponenten für die Wiederverwendung (CRU)", "lang": "de"}], "type": "flow data set", "refObjectId": "a2b32f97-3fc7-4af2-b209-525bc6426f33", "uri": "../flows/a2b32f97-3fc7-4af2-b209-525bc6426f33.xml"}, "exchange direction": "OUTPUT", "other": {"anies": [{"name": "referenceToUnitGroupDataSet", "value": {"shortDescription": [{"value": "kg", "lang": "en"}], "type": "unit group data set", "refObjectId": "ad38d542-3fe9-439d-9b95-2f5f7752acaf", "uri": "../unitgroups/ad38d542-3fe9-439d-9b95-2f5f7752acaf.xml"}}, {"value": "0", "module": "A1"}, {"value": "0", "module": "A2"}, {"value": "0", "module": "A3"}, {"value": "0", "module": "A4"}, {"value": "0", "module": "A5"}, {"value": "0", "module": "B6"}, {"value": "0", "module": "C1"}, {"value": "0", "module": "C2"}, {"value": "0", "module": "C3"}, {"value": "0", "module": "C4"}, {"value": "0", "module": "D"}]}, "resolvedFlowVersion": "38.00.000", "flowProperties": [], "typeOfFlow": "Other flow", "classification": {"classHierarchy": "Quantities / Environmental quantities / EPD EN 15804 / LCI indicators", "name": "GaBiCategories"}}, {"dataSetInternalID": 15, "referenceToFlowDataSet": {"shortDescription": [{"value": "Materials for recycling (MFR)", "lang": "en"}, {"value": "Stoffe zum Recycling (MFR)", "lang": "de"}], "type": "flow data set", "refObjectId": "d7fe48a5-4103-49c8-9aae-b0b5dfdbd6ae", "uri": "../flows/d7fe48a5-4103-49c8-9aae-b0b5dfdbd6ae.xml"}, "exchange direction": "OUTPUT", "other": {"anies": [{"name": "referenceToUnitGroupDataSet", "value": {"shortDescription": [{"value": "kg", "lang": "en"}], "type": "unit group data set", "refObjectId": "ad38d542-3fe9-439d-9b95-2f5f7752acaf", "uri": "../unitgroups/ad38d542-3fe9-439d-9b95-2f5f7752acaf.xml"}}, {"value": "0", "module": "A1"}, {"value": "0", "module": "A2"}, {"value": "0", "module": "A3"}, {"value": "0", "module": "A4"}, {"value": "0", "module": "A5"}, {"value": "0", "module": "B6"}, {"value": "0", "module": "C1"}, {"value": "0", "module": "C2"}, {"value": "18.98106337", "module": "C3"}, {"value": "0", "module": "C4"}, {"value": "0", "module": "D"}]}, "resolvedFlowVersion": "38.00.000", "flowProperties": [], "typeOfFlow": "Other flow", "classification": {"classHierarchy": "Quantities / Environmental quantities / EPD EN 15804 / LCI indicators", "name": "GaBiCategories"}}, {"dataSetInternalID": 16, "referenceToFlowDataSet": {"shortDescription": [{"value": "Materials for energy recovery (MER)", "lang": "en"}, {"value": "Stoffe für die Energierückgewinnung (MER)", "lang": "de"}], "type": "flow data set", "refObjectId": "59a9181c-3aaf-46ee-8b13-2b3723b6e447", "uri": "../flows/59a9181c-3aaf-46ee-8b13-2b3723b6e447.xml"}, "exchange direction": "OUTPUT", "other": {"anies": [{"name": "referenceToUnitGroupDataSet", "value": {"shortDescription": [{"value": "kg", "lang": "en"}], "type": "unit group data set", "refObjectId": "ad38d542-3fe9-439d-9b95-2f5f7752acaf", "uri": "../unitgroups/ad38d542-3fe9-439d-9b95-2f5f7752acaf.xml"}}, {"value": "0", "module": "A1"}, {"value": "0", "module": "A2"}, {"value": "0", "module": "A3"}, {"value": "0", "module": "A4"}, {"value": "0", "module": "A5"}, {"value": "0", "module": "B6"}, {"value": "0", "module": "C1"}, {"value": "0", "module": "C2"}, {"value": "0", "module": "C3"}, {"value": "0", "module": "C4"}, {"value": "0", "module": "D"}]}, "resolvedFlowVersion": "38.00.000", "flowProperties": [], "typeOfFlow": "Other flow", "classification": {"classHierarchy": "Quantities / Environmental quantities / EPD EN 15804 / LCI indicators", "name": "GaBiCategories"}}, {"dataSetInternalID": 17, "referenceToFlowDataSet": {"shortDescription": [{"value": "Exported electrical energy (EEE)", "lang": "en"}, {"value": "Exportierte elektrische Energie (EEE)", "lang": "de"}], "type": "flow data set", "refObjectId": "4da0c987-2b76-40d6-9e9e-82a017aaaf29", "uri": "../flows/4da0c987-2b76-40d6-9e9e-82a017aaaf29.xml"}, "exchange direction": "OUTPUT", "other": {"anies": [{"name": "referenceToUnitGroupDataSet", "value": {"shortDescription": [{"value": "MJ", "lang": "en"}], "type": "unit group data set", "refObjectId": "93a60a57-a3c8-11da-a746-0800200c9a66", "uri": "../unitgroups/93a60a57-a3c8-11da-a746-0800200c9a66.xml"}}, {"value": "0", "module": "A1"}, {"value": "0", "module": "A2"}, {"value": "0", "module": "A3"}, {"value": "0", "module": "A4"}, {"value": "4.36516756", "module": "A5"}, {"value": "0", "module": "B6"}, {"value": "0", "module": "C1"}, {"value": "0", "module": "C2"}, {"value": "7.435970062", "module": "C3"}, {"value": "0", "module": "C4"}, {"value": "0", "module": "D"}]}, "resolvedFlowVersion": "38.00.000", "flowProperties": [], "typeOfFlow": "Other flow", "classification": {"classHierarchy": "Quantities / Environmental quantities / EPD EN 15804 / LCI indicators", "name": "GaBiCategories"}}, {"dataSetInternalID": 18, "referenceToFlowDataSet": {"shortDescription": [{"value": "Exported thermal energy (EET)", "lang": "en"}, {"value": "Exportierte thermische Energie (EET)", "lang": "de"}], "type": "flow data set", "refObjectId": "98daf38a-7a79-46d3-9a37-2b7bd0955810", "uri": "../flows/98daf38a-7a79-46d3-9a37-2b7bd0955810.xml"}, "exchange direction": "OUTPUT", "other": {"anies": [{"name": "referenceToUnitGroupDataSet", "value": {"shortDescription": [{"value": "MJ", "lang": "en"}], "type": "unit group data set", "refObjectId": "93a60a57-a3c8-11da-a746-0800200c9a66", "uri": "../unitgroups/93a60a57-a3c8-11da-a746-0800200c9a66.xml"}}, {"value": "0", "module": "A1"}, {"value": "0", "module": "A2"}, {"value": "0", "module": "A3"}, {"value": "0", "module": "A4"}, {"value": "7.914898038", "module": "A5"}, {"value": "0", "module": "B6"}, {"value": "0", "module": "C1"}, {"value": "0", "module": "C2"}, {"value": "13.40963782", "module": "C3"}, {"value": "0", "module": "C4"}, {"value": "0", "module": "D"}]}, "resolvedFlowVersion": "38.00.000", "flowProperties": [], "typeOfFlow": "Other flow", "classification": {"classHierarchy": "Quantities / Environmental quantities / EPD EN 15804 / LCI indicators", "name": "GaBiCategories"}}]}, "LCIAResults": {"LCIAResult": [{"referenceToLCIAMethodDataSet": {"shortDescription": [{"value": "Global Warming Potential total (GWP-total)", "lang": "en"}, {"value": "Globales Erwärmungspotenzial total (GWP-total)", "lang": "de"}], "type": "LCIA method data set", "refObjectId": "6a37f984-a4b3-458a-a20a-64418c145fa2", "uri": "../lciamethods/6a37f984-a4b3-458a-a20a-64418c145fa2.xml"}, "other": {"anies": [{"name": "referenceToUnitGroupDataSet", "value": {"shortDescription": [{"value": "kg CO_(2) eq", "lang": "en"}], "type": "unit group data set", "refObjectId": "1ebf3012-d0db-4de2-aefd-ef30cedb0be1", "uri": "../unitgroups/1ebf3012-d0db-4de2-aefd-ef30cedb0be1.xml"}}, {"value": "111.7970683", "module": "A1"}, {"value": "1.560724847", "module": "A2"}, {"value": "0.853215", "module": "A3"}, {"value": "1.64047039", "module": "A4"}, {"value": "2.855418567", "module": "A5"}, {"value": "1136.592425", "module": "B6"}, {"value": "0", "module": "C1"}, {"value": "0.676507247", "module": "C2"}, {"value": "6.908670973", "module": "C3"}, {"value": "0.156999985", "module": "C4"}, {"value": "-1.431438791", "module": "D"}]}}, {"referenceToLCIAMethodDataSet": {"shortDescription": [{"value": "Global Warming Potential fossil fuels (GWP-fossil)", "lang": "en"}, {"value": "Globales Erwärmungspotenzial fossil (GWP-fossil)", "lang": "de"}], "type": "LCIA method data set", "refObjectId": "5f635281-343e-44fb-83df-1971b155e6b6", "uri": "../lciamethods/5f635281-343e-44fb-83df-1971b155e6b6.xml"}, "other": {"anies": [{"name": "referenceToUnitGroupDataSet", "value": {"shortDescription": [{"value": "kg CO_(2) eq", "lang": "en"}], "type": "unit group data set", "refObjectId": "1ebf3012-d0db-4de2-aefd-ef30cedb0be1", "uri": "../unitgroups/1ebf3012-d0db-4de2-aefd-ef30cedb0be1.xml"}}, {"value": "111.1529823", "module": "A1"}, {"value": "1.551525891", "module": "A2"}, {"value": "4.097172698", "module": "A3"}, {"value": "1.630814958", "module": "A4"}, {"value": "0.153000033", "module": "A5"}, {"value": "1131.182379", "module": "B6"}, {"value": "0", "module": "C1"}, {"value": "0.672174249", "module": "C2"}, {"value": "6.897767126", "module": "C3"}, {"value": "0.161726476", "module": "C4"}, {"value": "-1.428976427", "module": "D"}]}}, {"referenceToLCIAMethodDataSet": {"shortDescription": [{"value": "Global Warming Potential biogenic (GWP-biogenic)", "lang": "en"}, {"value": "Globales Erwärmungspotenzial biogen (GWP-biogenic)", "lang": "de"}], "type": "LCIA method data set", "refObjectId": "2356e1ab-0185-4db5-86e5-16de51c7485c", "uri": "../lciamethods/2356e1ab-0185-4db5-86e5-16de51c7485c.xml"}, "other": {"anies": [{"name": "referenceToUnitGroupDataSet", "value": {"shortDescription": [{"value": "kg CO_(2) eq", "lang": "en"}], "type": "unit group data set", "refObjectId": "1ebf3012-d0db-4de2-aefd-ef30cedb0be1", "uri": "../unitgroups/1ebf3012-d0db-4de2-aefd-ef30cedb0be1.xml"}}, {"value": "0.456066591", "module": "A1"}, {"value": "-0.002152769", "module": "A2"}, {"value": "-3.280628007", "module": "A3"}, {"value": "-0.003260139", "module": "A4"}, {"value": "2.702321606", "module": "A5"}, {"value": "3.770751168", "module": "B6"}, {"value": "0", "module": "C1"}, {"value": "-0.001133793", "module": "C2"}, {"value": "0.007287449", "module": "C3"}, {"value": "-0.004868399", "module": "C4"}, {"value": "0.001848153", "module": "D"}]}}, {"referenceToLCIAMethodDataSet": {"shortDescription": [{"value": "Global Warming Potential luluc (GWP-luluc)", "lang": "en"}, {"value": "Globales Erwärmungspotenzial luluc (GWP-luluc)", "lang": "de"}], "type": "LCIA method data set", "refObjectId": "4331bbdb-978a-490d-8707-eeb047f01a55", "uri": "../lciamethods/4331bbdb-978a-490d-8707-eeb047f01a55.xml"}, "other": {"anies": [{"name": "referenceToUnitGroupDataSet", "value": {"shortDescription": [{"value": "kg CO_(2) eq", "lang": "en"}], "type": "unit group data set", "refObjectId": "1ebf3012-d0db-4de2-aefd-ef30cedb0be1", "uri": "../unitgroups/1ebf3012-d0db-4de2-aefd-ef30cedb0be1.xml"}}, {"value": "0.188019378", "module": "A1"}, {"value": "0.011351725", "module": "A2"}, {"value": "0.03667031", "module": "A3"}, {"value": "0.012915572", "module": "A4"}, {"value": "9.69E-05", "module": "A5"}, {"value": "1.63929512", "module": "B6"}, {"value": "0", "module": "C1"}, {"value": "0.005466792", "module": "C2"}, {"value": "0.003616399", "module": "C3"}, {"value": "0.000141908", "module": "C4"}, {"value": "-0.004310517", "module": "D"}]}}, {"referenceToLCIAMethodDataSet": {"shortDescription": [{"value": "Depletion potential of the stratospheric ozone layer (ODP)", "lang": "en"}, {"value": "Abbau Potential der stratosphärischen Ozonschicht (ODP)", "lang": "de"}], "type": "LCIA method data set", "refObjectId": "b5c629d6-def3-11e6-bf01-fe55135034f3", "uri": "../lciamethods/b5c629d6-def3-11e6-bf01-fe55135034f3.xml"}, "other": {"anies": [{"name": "referenceToUnitGroupDataSet", "value": {"shortDescription": [{"value": "kg CFC11 eq", "lang": "en"}], "type": "unit group data set", "refObjectId": "d9e957c9-7309-4474-bf3a-7777df6c4e5b", "uri": "../unitgroups/d9e957c9-7309-4474-bf3a-7777df6c4e5b.xml"}}, {"value": "9.52E-08", "module": "A1"}, {"value": "2.72E-16", "module": "A2"}, {"value": "4.07E-09", "module": "A3"}, {"value": "1.99E-11", "module": "A4"}, {"value": "5.23E-16", "module": "A5"}, {"value": "2.49E-11", "module": "B6"}, {"value": "0", "module": "C1"}, {"value": "1.24E-16", "module": "C2"}, {"value": "5.45E-14", "module": "C3"}, {"value": "3.63E-16", "module": "C4"}, {"value": "-9.19E-13", "module": "D"}]}}, {"referenceToLCIAMethodDataSet": {"shortDescription": [{"value": "Acidification potential of land and water (AP)", "lang": "en"}, {"value": "Versauerungspotenzial von Boden und Wasser (AP)", "lang": "de"}], "type": "LCIA method data set", "refObjectId": "b5c611c6-def3-11e6-bf01-fe55135034f3", "uri": "../lciamethods/b5c611c6-def3-11e6-bf01-fe55135034f3.xml"}, "other": {"anies": [{"name": "referenceToUnitGroupDataSet", "value": {"shortDescription": [{"value": "mol H^(+) eq", "lang": "en"}], "type": "unit group data set", "refObjectId": "42e089ac-92bf-4bf2-8ca1-5fc40d18f2ed", "uri": "../unitgroups/42e089ac-92bf-4bf2-8ca1-5fc40d18f2ed.xml"}}, {"value": "0.60812002", "module": "A1"}, {"value": "0.011068079", "module": "A2"}, {"value": "0.017312648", "module": "A3"}, {"value": "0.009489486", "module": "A4"}, {"value": "0.000821905", "module": "A5"}, {"value": "2.497121738", "module": "B6"}, {"value": "0", "module": "C1"}, {"value": "0.003972009", "module": "C2"}, {"value": "0.006202088", "module": "C3"}, {"value": "0.000501779", "module": "C4"}, {"value": "-0.025229093", "module": "D"}]}}, {"referenceToLCIAMethodDataSet": {"shortDescription": [{"value": "Eutrophication potential aquatic freshwater (EP-freshwater)", "lang": "en"}, {"value": "Eutrophierungspotenzial Süßwasser (EP-freshwater)", "lang": "de"}], "type": "LCIA method data set", "refObjectId": "b53ec18f-7377-4ad3-86eb-cc3f4f276b2b", "uri": "../lciamethods/b53ec18f-7377-4ad3-86eb-cc3f4f276b2b.xml"}, "other": {"anies": [{"name": "referenceToUnitGroupDataSet", "value": {"shortDescription": [{"value": "kg P eq", "lang": "en"}], "type": "unit group data set", "refObjectId": "0429039d-a61d-4590-ba67-aa4a20a810a1", "uri": "../unitgroups/0429039d-a61d-4590-ba67-aa4a20a810a1.xml"}}, {"value": "0.001632696", "module": "A1"}, {"value": "4.31E-06", "module": "A2"}, {"value": "6.45E-05", "module": "A3"}, {"value": "5.21E-06", "module": "A4"}, {"value": "1.2E-07", "module": "A5"}, {"value": "0.003021373", "module": "B6"}, {"value": "0", "module": "C1"}, {"value": "2.06E-06", "module": "C2"}, {"value": "9.57E-06", "module": "C3"}, {"value": "1.76E-05", "module": "C4"}, {"value": "-5.04E-06", "module": "D"}]}}, {"referenceToLCIAMethodDataSet": {"shortDescription": [{"value": "Eutrophication potential aquatic marine (EP-marine)", "lang": "en"}, {"value": "Eutrophierungspotenzial Salzwasser (EP-marine)", "lang": "de"}], "type": "LCIA method data set", "refObjectId": "b5c619fa-def3-11e6-bf01-fe55135034f3", "uri": "../lciamethods/b5c619fa-def3-11e6-bf01-fe55135034f3.xml"}, "other": {"anies": [{"name": "referenceToUnitGroupDataSet", "value": {"shortDescription": [{"value": "kg N eq", "lang": "en"}], "type": "unit group data set", "refObjectId": "d05bb823-ecdf-4686-8c40-bf1d9257859f", "uri": "../unitgroups/d05bb823-ecdf-4686-8c40-bf1d9257859f.xml"}}, {"value": "0.076084694", "module": "A1"}, {"value": "0.003858971", "module": "A2"}, {"value": "0.003328087", "module": "A3"}, {"value": "0.004529766", "module": "A4"}, {"value": "0.000300106", "module": "A5"}, {"value": "0.554684579", "module": "B6"}, {"value": "0", "module": "C1"}, {"value": "0.001915922", "module": "C2"}, {"value": "0.00148775", "module": "C3"}, {"value": "0.000115785", "module": "C4"}, {"value": "-0.001312939", "module": "D"}]}}, {"referenceToLCIAMethodDataSet": {"shortDescription": [{"value": "Eutrophication potential terrestrial (EP-terrestrial)", "lang": "en"}, {"value": "Eutrophierungspotenzial Land (EP-terrestrial)", "lang": "de"}], "type": "LCIA method data set", "refObjectId": "b5c614d2-def3-11e6-bf01-fe55135034f3", "uri": "../lciamethods/b5c614d2-def3-11e6-bf01-fe55135034f3.xml"}, "other": {"anies": [{"name": "referenceToUnitGroupDataSet", "value": {"shortDescription": [{"value": "mol N eq", "lang": "en"}], "type": "unit group data set", "refObjectId": "71b4d617-0ec9-4d3f-b65e-e438940c2401", "uri": "../unitgroups/71b4d617-0ec9-4d3f-b65e-e438940c2401.xml"}}, {"value": "0.800267498", "module": "A1"}, {"value": "0.042740082", "module": "A2"}, {"value": "0.033345494", "module": "A3"}, {"value": "0.050154716", "module": "A4"}, {"value": "0.003728894", "module": "A5"}, {"value": "5.827550925", "module": "B6"}, {"value": "0", "module": "C1"}, {"value": "0.021218529", "module": "C2"}, {"value": "0.016545858", "module": "C3"}, {"value": "0.001270153", "module": "C4"}, {"value": "-0.013628046", "module": "D"}]}}, {"referenceToLCIAMethodDataSet": {"shortDescription": [{"value": "Formation potential of tropospheric ozone photochemical oxidants (POCP)", "lang": "en"}, {"value": "Bildungspotential für troposphärisches Ozon (POCP)", "lang": "de"}], "type": "LCIA method data set", "refObjectId": "b5c610fe-def3-11e6-bf01-fe55135034f3", "uri": "../lciamethods/b5c610fe-def3-11e6-bf01-fe55135034f3.xml"}, "other": {"anies": [{"name": "referenceToUnitGroupDataSet", "value": {"shortDescription": [{"value": "kg NMVOC eq", "lang": "en"}], "type": "unit group data set", "refObjectId": "d27c25f8-fbc1-44c6-b47b-4adbae4199c6", "uri": "../unitgroups/d27c25f8-fbc1-44c6-b47b-4adbae4199c6.xml"}}, {"value": "0.238175075", "module": "A1"}, {"value": "0.008857215", "module": "A2"}, {"value": "0.009552393", "module": "A3"}, {"value": "0.008621499", "module": "A4"}, {"value": "0.000783285", "module": "A5"}, {"value": "1.519780048", "module": "B6"}, {"value": "0", "module": "C1"}, {"value": "0.003635278", "module": "C2"}, {"value": "0.004068315", "module": "C3"}, {"value": "0.000372514", "module": "C4"}, {"value": "-0.00475732", "module": "D"}]}}, {"referenceToLCIAMethodDataSet": {"shortDescription": [{"value": "Abiotic depletion potential for non fossil resources (ADPE)", "lang": "en"}, {"value": "Potenzial für den abiotischen Abbau nicht fossiler Ressourcen (ADPE)", "lang": "de"}], "type": "LCIA method data set", "refObjectId": "b2ad6494-c78d-11e6-9d9d-cec0c932ce01", "uri": "../lciamethods/b2ad6494-c78d-11e6-9d9d-cec0c932ce01.xml"}, "other": {"anies": [{"name": "referenceToUnitGroupDataSet", "value": {"shortDescription": [{"value": "kg Sb eq", "lang": "en"}], "type": "unit group data set", "refObjectId": "54ccd2d9-a32a-4fc2-923d-f2c8c93e89d4", "uri": "../unitgroups/54ccd2d9-a32a-4fc2-923d-f2c8c93e89d4.xml"}}, {"value": "0.007506905", "module": "A1"}, {"value": "1.17E-07", "module": "A2"}, {"value": "6.1E-05", "module": "A3"}, {"value": "1.64E-06", "module": "A4"}, {"value": "8.71E-09", "module": "A5"}, {"value": "0.000327409", "module": "B6"}, {"value": "0", "module": "C1"}, {"value": "5.46E-08", "module": "C2"}, {"value": "7.17E-07", "module": "C3"}, {"value": "1.09E-08", "module": "C4"}, {"value": "-0.001258291", "module": "D"}]}}, {"referenceToLCIAMethodDataSet": {"shortDescription": [{"value": "Abiotic depletion potential for fossil resources (ADPF)", "lang": "en"}, {"value": "Potenzial für den abiotischen Abbau fossiler Brennstoffe (ADPF)", "lang": "de"}], "type": "LCIA method data set", "refObjectId": "b2ad6110-c78d-11e6-9d9d-cec0c932ce01", "uri": "../lciamethods/b2ad6110-c78d-11e6-9d9d-cec0c932ce01.xml"}, "other": {"anies": [{"name": "referenceToUnitGroupDataSet", "value": {"shortDescription": [{"value": "MJ", "lang": "en"}], "type": "unit group data set", "refObjectId": "93a60a57-a3c8-11da-a746-0800200c9a66", "uri": "../unitgroups/93a60a57-a3c8-11da-a746-0800200c9a66.xml"}}, {"value": "1490.705024", "module": "A1"}, {"value": "20.57202436", "module": "A2"}, {"value": "56.75720182", "module": "A3"}, {"value": "21.90756498", "module": "A4"}, {"value": "0.985306322", "module": "A5"}, {"value": "19885.48071", "module": "B6"}, {"value": "0", "module": "C1"}, {"value": "9.011083279", "module": "C2"}, {"value": "44.35420691", "module": "C3"}, {"value": "2.317610008", "module": "C4"}, {"value": "-26.69967579", "module": "D"}]}}, {"referenceToLCIAMethodDataSet": {"shortDescription": [{"value": "Water use (WDP)", "lang": "en"}, {"value": "Wassernutzung (WDP)", "lang": "de"}], "type": "LCIA method data set", "refObjectId": "b2ad66ce-c78d-11e6-9d9d-cec0c932ce01", "uri": "../lciamethods/b2ad66ce-c78d-11e6-9d9d-cec0c932ce01.xml"}, "other": {"anies": [{"name": "referenceToUnitGroupDataSet", "value": {"shortDescription": [{"value": "m^(3) world eq deprived", "lang": "en"}], "type": "unit group data set", "refObjectId": "6ae2df01-888e-46c8-b17d-49fa3869b476", "uri": "../unitgroups/6ae2df01-888e-46c8-b17d-49fa3869b476.xml"}}, {"value": "27.3297176", "module": "A1"}, {"value": "0.013948447", "module": "A2"}, {"value": "0.244503482", "module": "A3"}, {"value": "0.022462109", "module": "A4"}, {"value": "0.351803404", "module": "A5"}, {"value": "246.5579235", "module": "B6"}, {"value": "0", "module": "C1"}, {"value": "0.006585646", "module": "C2"}, {"value": "0.987521205", "module": "C3"}, {"value": "-0.001785381", "module": "C4"}, {"value": "-0.785416423", "module": "D"}]}}, {"referenceToLCIAMethodDataSet": {"shortDescription": [{"value": "Incidence of disease due to PM emissions (PM)", "lang": "en"}, {"value": "Auftreten von Krankheiten aufgrund von Feinstaubemissionen (PM)", "lang": "de"}], "type": "LCIA method data set", "refObjectId": "b5c602c6-def3-11e6-bf01-fe55135034f3", "uri": "../lciamethods/b5c602c6-def3-11e6-bf01-fe55135034f3.xml"}, "other": {"anies": [{"name": "referenceToUnitGroupDataSet", "value": {"shortDescription": [{"value": "Disease incidence", "lang": "en"}], "type": "unit group data set", "refObjectId": "3883559b-648f-4afc-8ba2-0bd24f3affa3", "uri": "../unitgroups/3883559b-648f-4afc-8ba2-0bd24f3affa3.xml"}}, {"value": "7.32E-06", "module": "A1"}, {"value": "1.29E-07", "module": "A2"}, {"value": "2.42E-07", "module": "A3"}, {"value": "5.64E-08", "module": "A4"}, {"value": "4.65E-09", "module": "A5"}, {"value": "2.09E-05", "module": "B6"}, {"value": "0", "module": "C1"}, {"value": "2.32E-08", "module": "C2"}, {"value": "5.24E-08", "module": "C3"}, {"value": "5.11E-09", "module": "C4"}, {"value": "-4.01E-07", "module": "D"}]}}, {"referenceToLCIAMethodDataSet": {"shortDescription": [{"value": "Human exposure efficiency relative to U235 (IR)", "lang": "en"}, {"value": "Wirkung durch Exposition des Menschen mit U235 (IR)", "lang": "de"}], "type": "LCIA method data set", "refObjectId": "b5c632be-def3-11e6-bf01-fe55135034f3", "uri": "../lciamethods/b5c632be-def3-11e6-bf01-fe55135034f3.xml"}, "other": {"anies": [{"name": "referenceToUnitGroupDataSet", "value": {"shortDescription": [{"value": "kBq U235 eq", "lang": "en"}], "type": "unit group data set", "refObjectId": "456b05bf-1415-44a9-9993-02452f554c09", "uri": "../unitgroups/456b05bf-1415-44a9-9993-02452f554c09.xml"}}, {"value": "6.862178687", "module": "A1"}, {"value": "0.005406266", "module": "A2"}, {"value": "0.246693313", "module": "A3"}, {"value": "0.008139256", "module": "A4"}, {"value": "0.007298659", "module": "A5"}, {"value": "495.147867", "module": "B6"}, {"value": "0", "module": "C1"}, {"value": "0.002459957", "module": "C2"}, {"value": "1.078567416", "module": "C3"}, {"value": "0.003940207", "module": "C4"}, {"value": "-0.027593699", "module": "D"}]}}, {"referenceToLCIAMethodDataSet": {"shortDescription": [{"value": "Comparative toxic unit for ecosystems (ETP-fw)", "lang": "en"}, {"value": "Toxizitätsvergleichseinheit für Ökosysteme (ETP-fw)", "lang": "de"}], "type": "LCIA method data set", "refObjectId": "ee1082d1-b0f7-43ca-a1f0-21e2a4a74511", "uri": "../lciamethods/ee1082d1-b0f7-43ca-a1f0-21e2a4a74511.xml"}, "other": {"anies": [{"name": "referenceToUnitGroupDataSet", "value": {"shortDescription": [{"value": "CTUe", "lang": "en"}], "type": "unit group data set", "refObjectId": "aa959ded-f1eb-4efb-9c5c-2d60be36b3e6", "uri": "../unitgroups/aa959ded-f1eb-4efb-9c5c-2d60be36b3e6.xml"}}, {"value": "871.7065238", "module": "A1"}, {"value": "15.31614966", "module": "A2"}, {"value": "18.4420756", "module": "A3"}, {"value": "16.07266973", "module": "A4"}, {"value": "0.497093933", "module": "A5"}, {"value": "8506.583771", "module": "B6"}, {"value": "0", "module": "C1"}, {"value": "6.74270082", "module": "C2"}, {"value": "19.27097517", "module": "C3"}, {"value": "1.632600028", "module": "C4"}, {"value": "-12.90605407", "module": "D"}]}}, {"referenceToLCIAMethodDataSet": {"shortDescription": [{"value": "Comparative toxic unit for humans (carcinogenic) (HTP-c)", "lang": "en"}, {"value": "Toxizitätsvergleichseinheit für Menschen (krebserregend) (HTP-c)", "lang": "de"}], "type": "LCIA method data set", "refObjectId": "2299222a-bbd8-474f-9d4f-4dd1f18aea7c", "uri": "../lciamethods/2299222a-bbd8-474f-9d4f-4dd1f18aea7c.xml"}, "other": {"anies": [{"name": "referenceToUnitGroupDataSet", "value": {"shortDescription": [{"value": "CTUh", "lang": "en"}], "type": "unit group data set", "refObjectId": "d4c9523e-2d7e-49fd-8469-998f547d3a70", "uri": "../unitgroups/d4c9523e-2d7e-49fd-8469-998f547d3a70.xml"}}, {"value": "1.65E-06", "module": "A1"}, {"value": "3.14E-10", "module": "A2"}, {"value": "6.65E-07", "module": "A3"}, {"value": "7.98E-10", "module": "A4"}, {"value": "2.44E-11", "module": "A5"}, {"value": "2.35E-07", "module": "B6"}, {"value": "0", "module": "C1"}, {"value": "1.4E-10", "module": "C2"}, {"value": "5.8E-10", "module": "C3"}, {"value": "9.36E-11", "module": "C4"}, {"value": "-7.02E-08", "module": "D"}]}}, {"referenceToLCIAMethodDataSet": {"shortDescription": [{"value": "Comparative toxic unit for humans (noncarcinogenic) (HTP-nc)", "lang": "en"}, {"value": "Toxizitätsvergleichseinheit für Menschen (nicht krebserregend) (HTP-nc)", "lang": "de"}], "type": "LCIA method data set", "refObjectId": "3af763a5-b7a1-48c9-9cee-1f223481fcef", "uri": "../lciamethods/3af763a5-b7a1-48c9-9cee-1f223481fcef.xml"}, "other": {"anies": [{"name": "referenceToUnitGroupDataSet", "value": {"shortDescription": [{"value": "CTUh", "lang": "en"}], "type": "unit group data set", "refObjectId": "d4c9523e-2d7e-49fd-8469-998f547d3a70", "uri": "../unitgroups/d4c9523e-2d7e-49fd-8469-998f547d3a70.xml"}}, {"value": "2.66E-06", "module": "A1"}, {"value": "1.71E-08", "module": "A2"}, {"value": "5.75E-08", "module": "A3"}, {"value": "1.95E-08", "module": "A4"}, {"value": "1.15E-09", "module": "A5"}, {"value": "8.66E-06", "module": "B6"}, {"value": "0", "module": "C1"}, {"value": "8E-09", "module": "C2"}, {"value": "2.32E-08", "module": "C3"}, {"value": "8.16E-09", "module": "C4"}, {"value": "-1.74E-08", "module": "D"}]}}, {"referenceToLCIAMethodDataSet": {"shortDescription": [{"value": "Soil quality index (SQP)", "lang": "en"}, {"value": "Bodenqualitätsindex (SQP)", "lang": "de"}], "type": "LCIA method data set", "refObjectId": "b2ad6890-c78d-11e6-9d9d-cec0c932ce01", "uri": "../lciamethods/b2ad6890-c78d-11e6-9d9d-cec0c932ce01.xml"}, "other": {"anies": [{"name": "referenceToUnitGroupDataSet", "value": {"shortDescription": [{"value": "SQP", "lang": "en"}], "type": "unit group data set", "refObjectId": "f130951c-e67f-4f7f-8dd4-665de3974e18", "uri": "../unitgroups/f130951c-e67f-4f7f-8dd4-665de3974e18.xml"}}, {"value": "438.8485339", "module": "A1"}, {"value": "6.57104387", "module": "A2"}, {"value": "97.20333409", "module": "A3"}, {"value": "7.585950939", "module": "A4"}, {"value": "0.267669927", "module": "A5"}, {"value": "6333.419489", "module": "B6"}, {"value": "0", "module": "C1"}, {"value": "3.162992902", "module": "C2"}, {"value": "13.98627724", "module": "C3"}, {"value": "0.16744485", "module": "C4"}, {"value": "-23.30630053", "module": "D"}]}}]}, "otherAttributes": {"{http://www.indata.network/EPD/2019}epd-version": "1.2"}, "version": "1.1", "locations": "../ILCDLocations.xml"}