{"processInformation": {"dataSetInformation": {"UUID": "7a5b7a61-c1da-44d7-9d25-0a9ce2c06088", "name": {"baseName": [{"value": "Superflor II, Needled tiles with a total pile weight of 521 g/m² and a CQuest Bio backing", "lang": "en"}, {"value": "Superflor II, genadelte Teppichfliesen mit einem Nutzschichtgewicht von 521 g/m2 und einer CQuest Bio Rückenbeschichtung", "lang": "de"}], "functionalUnitFlowProperties": [{"lang": "en"}]}, "classificationInformation": {"classification": [{"class": [{"value": "Kunststoffe", "level": 0, "classId": "6"}, {"value": "Bodenbeläge", "level": 1, "classId": "6.2"}, {"value": "Textile Bodenbeläge", "level": 2, "classId": "6.2.05"}], "name": "OEKOBAU.DAT"}, {"class": [{"value": "02 Building products", "level": 0}, {"value": "Floor coverings", "level": 1}, {"value": "Floor coverings", "level": 2}], "name": "IBUCategories"}]}, "generalComment": [{"value": "The declaration applies to needled carpet tiles having a surface pile of mainly solution-dyed PA 6, PP and PET with a total pile weight of 521 g/m2. The backing of the carpet consists of a CQuest Bio heavy backing covered by a polypropylene felt. The total recycled content of the carpet is 62%.\nCQuest Bio backing system:\n Backing compound based on renewable wood resin, containing a recycled\nfiller and glass-fleece reinforcement.", "lang": "en"}, {"value": "Die Deklaration gilt für genadelte Teppichfliesen mit einem Oberflächenflor aus hauptsächlich lösungsgefärbtem PA 6, PP und PET mit einem Gesamtflorgewicht von 521 g/m2. Der Teppichrücken besteht aus einem schweren CQuest Bio-Rücken, der mit einem Polypropylen-Filz abgedeckt ist. Der Gesamtanteil an recyceltem Material beträgt 62%. CQuest Bio Rückensystem: Rückenbeschichtung auf der Basis von erneuerbarem Holzharz, die einen recycelten Füllstoff und eine Glasvliesverstärkung enthält.", "lang": "de"}], "other": {"anies": [{"scenario": [{"description": [{"value": "100% landfill", "lang": "en"}, {"value": "100% Deponie", "lang": "de"}], "name": "S1", "default": true}, {"description": [{"value": "100% MWA", "lang": "en"}, {"value": "100% MVA", "lang": "de"}], "name": "S2"}, {"description": [{"value": "100% recovery in the cement industry", "lang": "en"}, {"value": "100% Rückgewinnung in der Zementindustrie", "lang": "de"}], "name": "S3"}]}]}}, "quantitativeReference": {"referenceToReferenceFlow": [0]}, "time": {"referenceYear": 2023, "dataSetValidUntil": 2028, "other": {"anies": [{"name": "publicationDateOfEPD", "value": 1683763200000}]}}, "geography": {"locationOfOperationSupplyOrProduction": {"location": "RER"}}, "technology": {"technologyDescriptionAndIncludedProcesses": [{"value": "Needled modular carpet tiles having a pile material of polyamide 6, polypropylene and polyester yarn from 87% recycled content with a PP felt covered heavy backing", "lang": "en"}, {"value": "Genadelte modulare Teppichfliesen mit einem Polmaterial aus Polyamid 6, Polypropylen und Polyestergarn aus 87% recyceltem Material und einem mit PP-Filz überzogenen schweren Rücken \nTechnische Daten: \nProdukt Form: Modulare Teppichfliesen (50cm x 50cm)\nArt der Herstellung: Genadelter Teppichboden\nFärbemethode: spinngefärbtes Garn\nGarntyp: PA6, PP, PET\nZweitrücken: CQB Schwerbeschichtung mit Abdeckvlies\nOberseitengewichtsatzgewicht:  521 g/m²\nGesamtgewicht des Teppichs: 4045 g/m² \n \nDeklarierte Einheit: \nDie angegebene Einheit bezieht sich auf 1 m²  produzierten textilen Bodenbelag. Der Output von Modul A5 \"Montage\" ist 1 m² verlegter textiler Bodenbelag. Die Rohdichte beträgt 586 g/m².", "lang": "de"}], "technologicalApplicability": [{"value": "The use class of the specific product as defined in EN 1307 can be found in the Product Information System (PRODIS) using the PRODIS registration number of the product.", "lang": "en"}, {"value": "Die in EN 1307 definierte Verwendungsklasse des jeweiligen Produkts finden Sie im Produktinformationssystem (PRODIS) unter Verwendung der PRODIS-Registrierungsnummer des Produkts.", "lang": "de"}]}}, "modellingAndValidation": {"LCIMethodAndAllocation": {"typeOfDataSet": "EPD", "referenceToLCAMethodDetails": [{"shortDescription": [{"value": "Floor coverings.pdf", "lang": "en"}], "type": "source data set", "refObjectId": "e95f60f8-9c2d-4e44-b6c6-716ed4859a57"}], "other": {"anies": [{"name": "subType", "value": "specific dataset"}]}}, "dataSourcesTreatmentAndRepresentativeness": {"referenceToDataSource": [{"shortDescription": [{"value": "GaBi Database (all versions)", "lang": "en"}], "type": "source data set", "refObjectId": "28d74cc0-db8b-4d7e-bc44-5f6d56ce0c4a"}, {"shortDescription": [{"value": "GaBi Database Edition 2022, CUP 2022.01", "lang": "en"}], "type": "source data set", "refObjectId": "86f664e2-7dab-4722-aad7-4c5206a4123b"}], "useAdviceForDataSet": [{"value": "Scope: \nThe manufacturer declaration applies to needled carpet tiles with a polypropylene felt covered heavy backing, a pile material of PA 6, PP and PET with a maximum total pile weight of 521 g/m2. The products are needled in Genemuiden, the Netherlands. The carpets are back coated in Scherpenzeel.\nThe declaration is only valid in conjunction with a valid GUT-PRODIS license of the product. \nSystem boundary: \nType of EPD: Cradle-to-gate with options\nSystem boundaries of modules A, B, C, D:\nModules C3, C4 and D are indicated separately for three end-of-life scenarios:\n1 - landfill disposal\n2 - municipal waste incineration\n3 - recovery in a cement plant\nA1-A3 Production:\nEnergysupply and production of the basic material, processing of secondary material, auxiliary material, transport of the material to the manufacturing site, emissions, waste water treatment, packaging material and waste processing up to the landfill disposal of residual waste (except radioactive waste). Benefits for generated electricity and steam due to the incineration of production waste are aggregated. Biogenic carbon that is stored in renewable material (wood resin, renewable additives,packaging paper) is taken into account as well as the associated carbon dioxide uptake from the air from which this biogenic carbon comes.\nA4 Transport:\nTransport of the packed textile floor covering from factory gate to the place of installation.\nA5 Installation:\nInstallation of the textile floor covering, processing of installation waste and packaging waste up to the landfill disposal of residual waste (except radioactive waste), the production of the amount of carpet that occurs as installation waste including its transport to the place of\ninstallation.\nGenerated electricity and steam due to the incineration of waste are listed in the result table as exported energy.\nBiogenic carbon that is stored in renewable materials in installation waste and packaging paper is released as carbon dioxide emissions into the air at the end of life in module A5.\nPreparation of the floor and auxiliary materials (adhesives, fixing agents, PET connectors) are beyond the system boundaries and not taken into account.\n\nB1 Use:\nIndoor emissions during the use stage. After the first year, no product-related Volatile Organic Compound (VOC) emissions are relevant due to known VOC decay curves of the product.\nB2 Maintenance:\nCleaning of the textile floor covering for a period of 1 year:\nVacuum cleaning – electricity supply Wet cleaning – electricity, water consumption, production of the cleaning agent, waste water treatment the declared values in this module have to be multiplied by the assumed service life of the floor covering in the building in question.\nB3 - B5:\nThe modules are not relevant within the assumed reference service life of 15 years.\nB6 - B7:\nNo energy and water input are required for the operation of the carpet in the use stage. The modules do not cause any environmental impact.\n\nC1 De-construction:\nThe floor covering is de-constructed manually and no additional environmental impact is caused.\nC2 Transport:\nTransport of the carpet waste to a landfill, to the municipal waste incineration plant (MWI) or to the waste collection facility for recycling.\nC3 Waste processing:\nC3-1: Landfill disposal needs no waste processing. \nC3-2: Impact from waste incineration (plant with R1 > 0.6), generated electricity and steam are listed in the result table as exported energy.\nC3-3:\nCollection of the carpet waste for recovery in the cement industry,\nwaste processing (granulating), transport to the cement plant, emissions\nfrom the incineration.\nC4 Disposal\nC4-1: Impact from landfill disposal,\nC4-2: The carpet waste leaves the system in module C3-2,\nC4-3: The pre-processed carpet waste leaves the system in module C3-3.\n\nD Recycling potential:\nCalculated benefits result from materials exclusive secondary materials (net materials).\nD-A5: Benefits for generated energy due to incineration of packaging and installation waste (incineration plant with R1 > 0.6), \nD-1: Assuming that the chemically bound renewable materials in a landfill gas do not release landfill gas within 100 years, no benefits due to landfill dosposal of carpet waste at the\nend-of-life are taken into account,\nD-2: Benefits for generated energy due to incineration of carpet waste at the end-of-life (incineration plant with R1 > 0.6),\nD-3: Benefits for saved fossil energy and saved inorganic material due to recovery of the carpet in a cement plant.", "lang": "en"}, {"value": "Gültigkeitsbereich: \nDie Herstellererklärung gilt für genadelte Teppichfliesen mit einem mit Polypropylenfilz überzogenen schweren Rücken, einem Polmaterial aus PA 6, PP und PET mit einem maximalen Gesamtpolgewicht von 521 g/m2. Die Produkte werden in Genemuiden, den Niederlanden, genadelt. Die Teppiche werden in Scherpenzeel rückseitig beschichtet. Die Deklaration ist nur in Verbindung mit einer gültigen GUT-PRODIS-Lizenz des Produkts gültig. \nSystemgrenze: \nArt der EPD: Cradle-to-Gate mit Optionen Systemgrenzen der Module A, B, C, D: Die Module C3, C4 und D werden separat für drei End-of-Life-Szenarien angegeben: 1 - Deponierung 2 - Verbrennung von Siedlungsabfällen 3 - Verwertung in einem Zementwerk A1-A3 Produktion: Energieversorgung und Produktion des Grundstoffs, Verarbeitung von Sekundärmaterial, Hilfsstoffen, Transport des Materials zum Herstellungsort, Emissionen, Abwasserbehandlung, Verpackungsmaterial und Abfallverarbeitung bis hin zur Deponierung von Restmüll (außer radioaktivem Abfall). Leistungen für erzeugten Strom und Dampf aufgrund der Verbrennung von Produktionsabfällen werden aggregiert. Biogener Kohlenstoff, der in erneuerbarem Material (Holzharz, erneuerbare Zusatzstoffe, Verpackungspapier) gespeichert ist, wird ebenso berücksichtigt wie die damit verbundene Kohlendioxidaufnahme aus der Luft, aus der dieser biogene Kohlenstoff stammt.\n\nA4 Transport: Transport des verpackten textilen Bodenbelags vom Werkstor bis zum Verlegeort. A5 Verlegung: Verlegung des textilen Bodenbelags, Verarbeitung von Verlegeabfällen und Verpackungsabfällen bis zur Deponierung von Restabfällen (außer radioaktiven Abfällen), die Produktion der als Verlegeabfälle anfallenden Teppichbodenmenge einschließlich deren Transport zum Verlegeort.\nDie durch die Verbrennung von Abfällen erzeugte Elektrizität und der Dampf werden in der Ergebnistabelle als exportierte Energie aufgeführt. Biogener Kohlenstoff, der in erneuerbaren Materialien in Verlegeabfällen und Verpackungspapier gespeichert ist, wird am Ende der Lebensdauer in Modul A5 als Kohlendioxidemissionen in die Luft freigesetzt. Die Vorbereitung des Bodens und die Hilfsstoffe (Klebstoffe, Fixiermittel, PET-Verbindungsstücke) liegen außerhalb der Systemgrenzen und werden nicht berücksichtigt. B1 Nutzung: Innenraumemissionen während der Nutzungsphase. Nach dem ersten Jahr sind aufgrund der bekannten VOC-Zerfallskurven des Produkts keine produktbezogenen Emissionen flüchtiger organischer Verbindungen (VOC) mehr relevant. B2 Wartung: Reinigung des textilen Bodenbelags für einen Zeitraum von 1 Jahr: Staubsaugen - Stromversorgung Nassreinigung - Strom, Wasserverbrauch, Herstellung des Reinigungsmittels, Abwasseraufbereitung Die angegebenen Werte in diesem Modul müssen mit der angenommenen Nutzungsdauer des Bodenbelags in dem betreffenden Gebäude multipliziert werden.\nB3 - B5: Die Module sind innerhalb der angenommenen Referenznutzungsdauer von 15 Jahren nicht relevant. B6 - B7: Für den Betrieb des Teppichbodens in der Nutzungsphase ist kein Energie- und Wassereinsatz erforderlich. Die Module verursachen keine Umweltauswirkungen. C1 Rückbau: Der Rückbau des Bodenbelags erfolgt manuell und verursacht keine zusätzlichen Umweltauswirkungen. C2 Transport: Transport des Teppichabfalls zu einer Deponie, zur kommunalen Müllverbrennungsanlage (KVA) oder zur Abfallsammelstelle für das Recycling. C3 Abfallverarbeitung: C3-1: Die Deponierung erfordert keine Abfallverarbeitung. \nC3-2: Auswirkungen der Abfallverbrennung (Anlage mit R1 > 0,6), erzeugter Strom und Dampf werden in der Ergebnistabelle als exportierte Energie aufgeführt. C3-3: Sammlung der Teppichabfälle zur Verwertung in der Zementindustrie, Abfallverarbeitung (Granulierung), Transport zum Zementwerk, Emissionen aus der Verbrennung.\n\nC4 Entsorgung C4-1: Auswirkung der Deponierung, C4-2: Der Teppichabfall verlässt das System in Modul C3-2, C4-3: Der vorverarbeitete Teppichabfall verlässt das System in Modul C3-3. D Verwertungspotenzial: Der berechnete Nutzen ergibt sich aus den Materialien ohne Sekundärmaterialien (Nettomaterialien).\nD-A5: Nutzen für die erzeugte Energie durch die Verbrennung von Verpackungs- und Installationsabfällen (Verbrennungsanlage mit R1 > 0.6), D-1: Unter der Annahme, dass die chemisch gebundenen erneuerbaren Materialien in einem Deponiegas innerhalb von 100 Jahren kein Deponiegas freisetzen, wird kein Nutzen aufgrund der Deponierung von Teppichabfällen am Ende der Lebensdauer berücksichtigt, D-2: Nutzen für erzeugte Energie aufgrund der Verbrennung von Teppichabfällen am Ende der Lebensdauer (Verbrennungsanlage mit R1 > 0,6), D-3: Nutzen für eingesparte fossile Energie und eingespartes anorganisches Material aufgrund der Verwertung des Teppichs in einem Zementwerk.", "lang": "de"}], "other": {"anies": [{"name": "referenceToOriginalEPD", "value": {"shortDescription": {"value": "Superflor II, Needled tiles with a total pile weight of 521 g/m²  and a CQuest Bio backing.pdf", "defaultValue": "Superflor II, Needled tiles with a total pile weight of 521 g/m²  and a CQuest Bio backing.pdf", "lstrings": [{"lang": "en", "value": "Superflor II, Needled tiles with a total pile weight of 521 g/m²  and a CQuest Bio backing.pdf"}]}, "type": "source data set", "uuid": {"uuid": "81a7fd1a-1aa7-42db-9cf3-c077bc94c8c4"}, "refObjectId": "81a7fd1a-1aa7-42db-9cf3-c077bc94c8c4", "resourceURLs": ["https://oekobaudat.de/OEKOBAU.DAT/resource/sources/81a7fd1a-1aa7-42db-9cf3-c077bc94c8c4/Superflor_II_Needled_tiles_with_a_total_pile_weight_of_521_gm_and_a_CQuest_Bio_backing_18988.pdf?version=00.02.000"]}}]}}, "validation": {"review": [{"referenceToNameOfReviewerAndInstitution": [{"shortDescription": [{"value": "Institut Bauen und Umwelt e. V.", "lang": "en"}], "type": "contact data set", "refObjectId": "d111dbec-b024-4be5-86c5-752d6eb2cf95", "uri": "../contacts/d111dbec-b024-4be5-86c5-752d6eb2cf95.xml"}], "type": "Accredited third party review"}]}, "complianceDeclarations": {"compliance": [{"referenceToComplianceSystem": {"shortDescription": [{"value": "DIN EN 15804+A2", "lang": "en"}], "type": "source data set", "refObjectId": "c0016b33-8cf7-415c-ac6e-deba0d21440d", "uri": "../sources/c0016b33-8cf7-415c-ac6e-deba0d21440d.xml"}}, {"referenceToComplianceSystem": {"shortDescription": [{"value": "ISO 14025", "lang": "en"}], "type": "source data set", "refObjectId": "4f2eb655-6e44-4874-a95a-e28f5442cd4d", "uri": "../sources/4f2eb655-6e44-4874-a95a-e28f5442cd4d.xml"}}]}}, "administrativeInformation": {"commissionerAndGoal": {"referenceToCommissioner": [{"shortDescription": [{"value": "Interface Europe Manufacturing BV", "lang": "en"}], "type": "contact data set", "refObjectId": "bc3caa47-14fa-4575-8af1-da922eb46a69", "uri": "../contacts/bc3caa47-14fa-4575-8af1-da922eb46a69.xml"}]}, "dataGenerator": {"referenceToPersonOrEntityGeneratingTheDataSet": [{"shortDescription": [{"value": "Gemeinschaft umweltfreundlicher Teppichboden (GUT) e.V.", "lang": "en"}], "type": "contact data set", "refObjectId": "1e593d93-ef5b-4ddc-9b55-f58cf8960f3e", "uri": "../contacts/1e593d93-ef5b-4ddc-9b55-f58cf8960f3e.xml"}]}, "dataEntryBy": {"timeStamp": 1683763200000, "referenceToDataSetFormat": [{"shortDescription": [{"value": "ILCD Format", "lang": "en"}], "type": "source data set", "refObjectId": "a97a0155-0234-4b87-b4ce-a45da52f2a40", "uri": "../sources/a97a0155-0234-4b87-b4ce-a45da52f2a40.xml"}, {"shortDescription": [{"value": "EPD-Datenformaterweiterungen v1.2", "lang": "de"}, {"value": "EPD Data Format Extensions v1.2", "lang": "en"}], "type": "source data set", "refObjectId": "a29449fd-aa2f-4de8-b5d7-4b06b43c6fde", "uri": "../sources/a29449fd-aa2f-4de8-b5d7-4b06b43c6fde.xml"}]}, "publicationAndOwnership": {"dataSetVersion": "00.04.000", "referenceToPrecedingDataSetVersion": [{"shortDescription": [{"value": "Superflor II, Needled tiles with a total pile weight of 521 g/m2 and a CQuest Bio backing", "lang": "en"}], "type": "process data set", "refObjectId": "2729203b-36fb-467c-af82-675eedb033c9", "uri": "../processes/2729203b-36fb-467c-af82-675eedb033c9.xml"}], "referenceToRegistrationAuthority": {"shortDescription": [{"value": "Institut Bauen und Umwelt e. V.", "lang": "en"}], "type": "contact data set", "refObjectId": "d111dbec-b024-4be5-86c5-752d6eb2cf95", "uri": "../contacts/d111dbec-b024-4be5-86c5-752d6eb2cf95.xml"}, "registrationNumber": "EPD-INT-20220230-CBB3-EN", "referenceToOwnershipOfDataSet": {"shortDescription": [{"value": "Interface Europe Manufacturing BV", "lang": "en"}], "type": "contact data set", "refObjectId": "bc3caa47-14fa-4575-8af1-da922eb46a69", "uri": "../contacts/bc3caa47-14fa-4575-8af1-da922eb46a69.xml"}, "copyright": true, "licenseType": "Free of charge for all users and uses", "accessRestrictions": [{"value": "None", "lang": "en"}], "other": {"anies": [{"name": "referenceToPublisher", "value": {"shortDescription": [{"value": "Institut Bauen und Umwelt e. V.", "lang": "en"}], "type": "contact data set", "refObjectId": "d111dbec-b024-4be5-86c5-752d6eb2cf95", "uri": "../contacts/d111dbec-b024-4be5-86c5-752d6eb2cf95.xml"}}]}}}, "exchanges": {"exchange": [{"dataSetInternalID": 0, "referenceToFlowDataSet": {"shortDescription": [{"value": "Superflor II, Needled tiles with a total pile weight of 521 g/m² and a CQuest Bio backing (Superflor II, genadelte Teppichfliesen mit einem Nutzschichtgewicht von 521 g/m2 und einer CQuest Bio Rückenbeschichtung)", "lang": "en"}], "type": "flow data set", "refObjectId": "68ba4ee5-b00a-1681-6f8a-6517d2c2c105", "uri": "../flows/68ba4ee5-b00a-1681-6f8a-6517d2c2c105.xml"}, "meanAmount": 1.0, "referencesToDataSource": {}, "referenceFlow": true, "resolvedFlowVersion": "00.04.000", "resultingflowAmount": 1.0, "flowProperties": [{"name": [{"lang": "de", "value": "Fläche"}, {"lang": "en", "value": "Area"}], "uuid": "93a60a56-a3c8-19da-a746-0800200c9a66", "referenceFlowProperty": true, "meanValue": 1.0, "referenceUnit": "qm", "unitGroupUUID": "c20a03d7-bd90-4569-bc94-66cfd364dfc8"}], "materialProperties": [{"name": "gross density", "value": "586.0", "unit": "kg/m^3", "unitDescription": "kilograms per cubic metre"}, {"name": "grammage", "value": "4.045", "unit": "kg/m^2", "unitDescription": "kilograms per square meter"}, {"name": "layer thickness", "value": "0.0069", "unit": "m", "unitDescription": "meters"}], "typeOfFlow": "Product flow", "classification": {"classHierarchy": "Kunststoffe / Bodenbeläge / Textile Bodenbeläge", "name": "OEKOBAU.DAT"}}, {"dataSetInternalID": 1, "referenceToFlowDataSet": {"shortDescription": [{"value": "Renewable primary energy as energy carrier (PERE)", "lang": "en"}, {"value": "Erneuerbare Primärenergie als Energieträger (PERE)", "lang": "de"}], "type": "flow data set", "refObjectId": "20f32be5-0398-4288-9b6d-accddd195317", "uri": "../flows/20f32be5-0398-4288-9b6d-accddd195317.xml"}, "exchange direction": "INPUT", "other": {"anies": [{"name": "referenceToUnitGroupDataSet", "value": {"shortDescription": [{"value": "MJ", "lang": "en"}], "type": "unit group data set", "refObjectId": "93a60a57-a3c8-11da-a746-0800200c9a66", "uri": "../unitgroups/93a60a57-a3c8-11da-a746-0800200c9a66.xml"}}, {"value": "33.742", "module": "A1-A3"}, {"value": "0.1879", "module": "A4"}, {"value": "1.77158", "module": "A5"}, {"value": "0", "module": "B1"}, {"value": "3.685", "module": "B2"}, {"value": "0", "module": "C1"}, {"value": "0.0104", "module": "C2"}, {"value": "16.1544", "module": "C3", "scenario": "S2"}, {"value": "16.3891", "module": "C3", "scenario": "S3"}, {"value": "0.3344", "module": "C4"}, {"value": "-0.209", "module": "D"}, {"value": "0", "module": "D", "scenario": "S1"}, {"value": "-4.84", "module": "D", "scenario": "S2"}, {"value": "-0.2801", "module": "D", "scenario": "S3"}]}, "resolvedFlowVersion": "38.00.000", "flowProperties": [], "typeOfFlow": "Other flow", "classification": {"classHierarchy": "Quantities", "name": "GaBiCategories"}}, {"dataSetInternalID": 2, "referenceToFlowDataSet": {"shortDescription": [{"value": "Renewable primary energy resources as material utilization (PERM)", "lang": "en"}, {"value": "Erneuerbare Primärenergie zur stofflichen Nutzung (PERM)", "lang": "de"}], "type": "flow data set", "refObjectId": "fb3ec0de-548d-4508-aea5-00b73bf6f702", "uri": "../flows/fb3ec0de-548d-4508-aea5-00b73bf6f702.xml"}, "exchange direction": "INPUT", "other": {"anies": [{"name": "referenceToUnitGroupDataSet", "value": {"shortDescription": [{"value": "MJ", "lang": "en"}], "type": "unit group data set", "refObjectId": "93a60a57-a3c8-11da-a746-0800200c9a66", "uri": "../unitgroups/93a60a57-a3c8-11da-a746-0800200c9a66.xml"}}, {"value": "15.948", "module": "A1-A3"}, {"value": "0", "module": "A4"}, {"value": "-0.26", "module": "A5"}, {"value": "0", "module": "B1"}, {"value": "0", "module": "B2"}, {"value": "0", "module": "C1"}, {"value": "0", "module": "C2"}, {"value": "-15.688", "module": "C3", "scenario": "S2"}, {"value": "-15.688", "module": "C3", "scenario": "S3"}, {"value": "0", "module": "C4"}, {"value": "0", "module": "D"}, {"value": "0", "module": "D", "scenario": "S1"}, {"value": "0", "module": "D", "scenario": "S2"}, {"value": "0", "module": "D", "scenario": "S3"}]}, "resolvedFlowVersion": "38.00.000", "flowProperties": [], "typeOfFlow": "Other flow", "classification": {"classHierarchy": "Quantities", "name": "GaBiCategories"}}, {"dataSetInternalID": 3, "referenceToFlowDataSet": {"shortDescription": [{"value": "Total use of renewable primary energy resources (PERT)", "lang": "en"}, {"value": "Total erneuerbare Primärenergie (PERT)", "lang": "de"}], "type": "flow data set", "refObjectId": "53f97275-fa8a-4cdd-9024-65936002acd0", "uri": "../flows/53f97275-fa8a-4cdd-9024-65936002acd0.xml"}, "exchange direction": "INPUT", "other": {"anies": [{"name": "referenceToUnitGroupDataSet", "value": {"shortDescription": [{"value": "MJ", "lang": "en"}], "type": "unit group data set", "refObjectId": "93a60a57-a3c8-11da-a746-0800200c9a66", "uri": "../unitgroups/93a60a57-a3c8-11da-a746-0800200c9a66.xml"}}, {"value": "49.69", "module": "A1-A3"}, {"value": "0.1879", "module": "A4"}, {"value": "1.51158", "module": "A5"}, {"value": "0", "module": "B1"}, {"value": "3.685", "module": "B2"}, {"value": "0", "module": "C1"}, {"value": "0.0104", "module": "C2"}, {"value": "0.4664", "module": "C3", "scenario": "S2"}, {"value": "0.7011", "module": "C3", "scenario": "S3"}, {"value": "0.3344", "module": "C4"}, {"value": "-0.209", "module": "D"}, {"value": "0", "module": "D", "scenario": "S1"}, {"value": "-4.84", "module": "D", "scenario": "S2"}, {"value": "-0.2801", "module": "D", "scenario": "S3"}]}, "resolvedFlowVersion": "38.00.000", "flowProperties": [], "typeOfFlow": "Other flow", "classification": {"classHierarchy": "Quantities / Environmental quantities / EPD EN 15804 / LCI indicators", "name": "GaBiCategories"}}, {"dataSetInternalID": 4, "referenceToFlowDataSet": {"shortDescription": [{"value": "Non renewable primary energy as energy carrier (PENRE)", "lang": "en"}, {"value": "Nicht-erneuerbare Primärenergie als Energieträger (PENRE)", "lang": "de"}], "type": "flow data set", "refObjectId": "ac857178-2b45-46ec-892a-a9a4332f0372", "uri": "../flows/ac857178-2b45-46ec-892a-a9a4332f0372.xml"}, "exchange direction": "INPUT", "other": {"anies": [{"name": "referenceToUnitGroupDataSet", "value": {"shortDescription": [{"value": "MJ", "lang": "en"}], "type": "unit group data set", "refObjectId": "93a60a57-a3c8-11da-a746-0800200c9a66", "uri": "../unitgroups/93a60a57-a3c8-11da-a746-0800200c9a66.xml"}}, {"value": "128.981", "module": "A1-A3"}, {"value": "3.313", "module": "A4"}, {"value": "5.3839", "module": "A5"}, {"value": "0", "module": "B1"}, {"value": "5.898", "module": "B2"}, {"value": "0", "module": "C1"}, {"value": "0.1834", "module": "C2"}, {"value": "33.189", "module": "C3", "scenario": "S2"}, {"value": "34.024", "module": "C3", "scenario": "S3"}, {"value": "4.07", "module": "C4"}, {"value": "-0.7611", "module": "D"}, {"value": "0", "module": "D", "scenario": "S1"}, {"value": "-17.67", "module": "D", "scenario": "S2"}, {"value": "-40.9", "module": "D", "scenario": "S3"}]}, "resolvedFlowVersion": "38.00.000", "flowProperties": [], "typeOfFlow": "Other flow", "classification": {"classHierarchy": "Quantities", "name": "GaBiCategories"}}, {"dataSetInternalID": 5, "referenceToFlowDataSet": {"shortDescription": [{"value": "Non renewable primary energy as material utilization (PENRM)", "lang": "en"}, {"value": "Nicht-erneuerbare Primärenergie zur stofflichen Nutzung (PENRM)", "lang": "de"}], "type": "flow data set", "refObjectId": "1421caa0-679d-4bf4-b282-0eb850ccae27", "uri": "../flows/1421caa0-679d-4bf4-b282-0eb850ccae27.xml"}, "exchange direction": "INPUT", "other": {"anies": [{"name": "referenceToUnitGroupDataSet", "value": {"shortDescription": [{"value": "MJ", "lang": "en"}], "type": "unit group data set", "refObjectId": "93a60a57-a3c8-11da-a746-0800200c9a66", "uri": "../unitgroups/93a60a57-a3c8-11da-a746-0800200c9a66.xml"}}, {"value": "31.019", "module": "A1-A3"}, {"value": "0", "module": "A4"}, {"value": "-0.396", "module": "A5"}, {"value": "0", "module": "B1"}, {"value": "0", "module": "B2"}, {"value": "0", "module": "C1"}, {"value": "0", "module": "C2"}, {"value": "-30.623", "module": "C3", "scenario": "S2"}, {"value": "-30.623", "module": "C3", "scenario": "S3"}, {"value": "0", "module": "C4"}, {"value": "0", "module": "D"}, {"value": "0", "module": "D", "scenario": "S1"}, {"value": "0", "module": "D", "scenario": "S2"}, {"value": "0", "module": "D", "scenario": "S3"}]}, "resolvedFlowVersion": "38.00.000", "flowProperties": [], "typeOfFlow": "Other flow", "classification": {"classHierarchy": "Quantities", "name": "GaBiCategories"}}, {"dataSetInternalID": 6, "referenceToFlowDataSet": {"shortDescription": [{"value": "Total use of non renewable primary energy resources (PENRT)", "lang": "en"}, {"value": "Total nicht erneuerbare Primärenergie (PENRT)", "lang": "de"}], "type": "flow data set", "refObjectId": "06159210-646b-4c8d-8583-da9b3b95a6c1", "uri": "../flows/06159210-646b-4c8d-8583-da9b3b95a6c1.xml"}, "exchange direction": "INPUT", "other": {"anies": [{"name": "referenceToUnitGroupDataSet", "value": {"shortDescription": [{"value": "MJ", "lang": "en"}], "type": "unit group data set", "refObjectId": "93a60a57-a3c8-11da-a746-0800200c9a66", "uri": "../unitgroups/93a60a57-a3c8-11da-a746-0800200c9a66.xml"}}, {"value": "160", "module": "A1-A3"}, {"value": "3.313", "module": "A4"}, {"value": "4.9879", "module": "A5"}, {"value": "0", "module": "B1"}, {"value": "5.898", "module": "B2"}, {"value": "0", "module": "C1"}, {"value": "0.1834", "module": "C2"}, {"value": "2.566", "module": "C3", "scenario": "S2"}, {"value": "3.401", "module": "C3", "scenario": "S3"}, {"value": "4.07", "module": "C4"}, {"value": "-0.7611", "module": "D"}, {"value": "0", "module": "D", "scenario": "S1"}, {"value": "-17.67", "module": "D", "scenario": "S2"}, {"value": "-40.9", "module": "D", "scenario": "S3"}]}, "resolvedFlowVersion": "38.00.000", "flowProperties": [], "typeOfFlow": "Other flow", "classification": {"classHierarchy": "Quantities / Environmental quantities / EPD EN 15804 / LCI indicators", "name": "GaBiCategories"}}, {"dataSetInternalID": 7, "referenceToFlowDataSet": {"shortDescription": [{"value": "Use of secondary material (SM)", "lang": "en"}, {"value": "Einsatz von Sekundärstoffen (SM)", "lang": "de"}], "type": "flow data set", "refObjectId": "c6a1f35f-2d09-4f54-8dfb-97e502e1ce92", "uri": "../flows/c6a1f35f-2d09-4f54-8dfb-97e502e1ce92.xml"}, "exchange direction": "INPUT", "other": {"anies": [{"name": "referenceToUnitGroupDataSet", "value": {"shortDescription": [{"value": "kg", "lang": "en"}], "type": "unit group data set", "refObjectId": "ad38d542-3fe9-439d-9b95-2f5f7752acaf", "uri": "../unitgroups/ad38d542-3fe9-439d-9b95-2f5f7752acaf.xml"}}, {"value": "2.574", "module": "A1-A3"}, {"value": "0", "module": "A4"}, {"value": "0.07722", "module": "A5"}, {"value": "0", "module": "B1"}, {"value": "0", "module": "B2"}, {"value": "0", "module": "C1"}, {"value": "0", "module": "C2"}, {"value": "0", "module": "C3", "scenario": "S2"}, {"value": "0", "module": "C3", "scenario": "S3"}, {"value": "0", "module": "C4"}, {"value": "0", "module": "D"}, {"value": "0", "module": "D", "scenario": "S1"}, {"value": "0", "module": "D", "scenario": "S2"}, {"value": "0.02", "module": "D", "scenario": "S3"}]}, "resolvedFlowVersion": "38.00.000", "flowProperties": [], "typeOfFlow": "Other flow", "classification": {"classHierarchy": "Quantities / Environmental quantities / EPD EN 15804 / LCI indicators", "name": "GaBiCategories"}}, {"dataSetInternalID": 8, "referenceToFlowDataSet": {"shortDescription": [{"value": "Use of renewable secondary fuels (RSF)", "lang": "en"}, {"value": "Erneuerbare Sekundärbrennstoffe (RSF)", "lang": "de"}], "type": "flow data set", "refObjectId": "64333088-a55f-4aa2-9a31-c10b07816787", "uri": "../flows/64333088-a55f-4aa2-9a31-c10b07816787.xml"}, "exchange direction": "INPUT", "other": {"anies": [{"name": "referenceToUnitGroupDataSet", "value": {"shortDescription": [{"value": "MJ", "lang": "en"}], "type": "unit group data set", "refObjectId": "93a60a57-a3c8-11da-a746-0800200c9a66", "uri": "../unitgroups/93a60a57-a3c8-11da-a746-0800200c9a66.xml"}}, {"value": "0", "module": "A1-A3"}, {"value": "0", "module": "A4"}, {"value": "0", "module": "A5"}, {"value": "0", "module": "B1"}, {"value": "0", "module": "B2"}, {"value": "0", "module": "C1"}, {"value": "0", "module": "C2"}, {"value": "0", "module": "C3", "scenario": "S2"}, {"value": "0", "module": "C3", "scenario": "S3"}, {"value": "0", "module": "C4"}, {"value": "0", "module": "D"}, {"value": "0", "module": "D", "scenario": "S1"}, {"value": "0", "module": "D", "scenario": "S2"}, {"value": "0", "module": "D", "scenario": "S3"}]}, "resolvedFlowVersion": "38.00.000", "flowProperties": [], "typeOfFlow": "Other flow", "classification": {"classHierarchy": "Quantities / Environmental quantities / EPD EN 15804 / LCI indicators", "name": "GaBiCategories"}}, {"dataSetInternalID": 9, "referenceToFlowDataSet": {"shortDescription": [{"value": "Use of non renewable secondary fuels (NRSF)", "lang": "en"}, {"value": "Nicht erneuerbare Sekundärbrennstoffe (NRSF)", "lang": "de"}], "type": "flow data set", "refObjectId": "89def144-d39a-4287-b86f-efde453ddcb2", "uri": "../flows/89def144-d39a-4287-b86f-efde453ddcb2.xml"}, "exchange direction": "INPUT", "other": {"anies": [{"name": "referenceToUnitGroupDataSet", "value": {"shortDescription": [{"value": "MJ", "lang": "en"}], "type": "unit group data set", "refObjectId": "93a60a57-a3c8-11da-a746-0800200c9a66", "uri": "../unitgroups/93a60a57-a3c8-11da-a746-0800200c9a66.xml"}}, {"value": "0", "module": "A1-A3"}, {"value": "0", "module": "A4"}, {"value": "0", "module": "A5"}, {"value": "0", "module": "B1"}, {"value": "0", "module": "B2"}, {"value": "0", "module": "C1"}, {"value": "0", "module": "C2"}, {"value": "0", "module": "C3", "scenario": "S2"}, {"value": "0", "module": "C3", "scenario": "S3"}, {"value": "0", "module": "C4"}, {"value": "0", "module": "D"}, {"value": "0", "module": "D", "scenario": "S1"}, {"value": "0", "module": "D", "scenario": "S2"}, {"value": "0", "module": "D", "scenario": "S3"}]}, "resolvedFlowVersion": "38.00.000", "flowProperties": [], "typeOfFlow": "Other flow", "classification": {"classHierarchy": "Quantities / Environmental quantities / EPD EN 15804 / LCI indicators", "name": "GaBiCategories"}}, {"dataSetInternalID": 10, "referenceToFlowDataSet": {"shortDescription": [{"value": "Use of net fresh water (FW)", "lang": "en"}, {"value": "Einsatz von Süßwasserressourcen (FW)", "lang": "de"}], "type": "flow data set", "refObjectId": "3cf952c8-f3a4-461d-8c96-96456ca62246", "uri": "../flows/3cf952c8-f3a4-461d-8c96-96456ca62246.xml"}, "exchange direction": "INPUT", "other": {"anies": [{"name": "referenceToUnitGroupDataSet", "value": {"shortDescription": [{"value": "m^3", "lang": "en"}], "type": "unit group data set", "refObjectId": "cd950537-0a98-4044-9ba7-9f9a68d0a504", "uri": "../unitgroups/cd950537-0a98-4044-9ba7-9f9a68d0a504.xml"}}, {"value": "0.3685", "module": "A1-A3"}, {"value": "0.0002123", "module": "A4"}, {"value": "0.0115536", "module": "A5"}, {"value": "0", "module": "B1"}, {"value": "0.003344", "module": "B2"}, {"value": "0", "module": "C1"}, {"value": "1.175E-05", "module": "C2"}, {"value": "0.01431", "module": "C3", "scenario": "S2"}, {"value": "0.01454", "module": "C3", "scenario": "S3"}, {"value": "4.764E-05", "module": "C4"}, {"value": "-0.0001998", "module": "D"}, {"value": "0", "module": "D", "scenario": "S1"}, {"value": "-0.004625", "module": "D", "scenario": "S2"}, {"value": "-0.003554", "module": "D", "scenario": "S3"}]}, "resolvedFlowVersion": "38.00.000", "flowProperties": [], "typeOfFlow": "Other flow", "classification": {"classHierarchy": "Quantities / Environmental quantities / EPD EN 15804 / LCI indicators", "name": "GaBiCategories"}}, {"dataSetInternalID": 11, "referenceToFlowDataSet": {"shortDescription": [{"value": "Hazardous waste disposed (HWD)", "lang": "en"}, {"value": "Gefährlicher Abfall zur Deponie (HWD)", "lang": "de"}], "type": "flow data set", "refObjectId": "430f9e0f-59b2-46a0-8e0d-55e0e84948fc", "uri": "../flows/430f9e0f-59b2-46a0-8e0d-55e0e84948fc.xml"}, "exchange direction": "OUTPUT", "other": {"anies": [{"name": "referenceToUnitGroupDataSet", "value": {"shortDescription": [{"value": "kg", "lang": "en"}], "type": "unit group data set", "refObjectId": "ad38d542-3fe9-439d-9b95-2f5f7752acaf", "uri": "../unitgroups/ad38d542-3fe9-439d-9b95-2f5f7752acaf.xml"}}, {"value": "2.26E-07", "module": "A1-A3"}, {"value": "1.59E-11", "module": "A4"}, {"value": "6.7918E-09", "module": "A5"}, {"value": "0", "module": "B1"}, {"value": "4.19E-05", "module": "B2"}, {"value": "0", "module": "C1"}, {"value": "8.78E-13", "module": "C2"}, {"value": "3.67E-10", "module": "C3", "scenario": "S2"}, {"value": "4.02E-10", "module": "C3", "scenario": "S3"}, {"value": "6.27E-10", "module": "C4"}, {"value": "-1.03E-10", "module": "D"}, {"value": "0", "module": "D", "scenario": "S1"}, {"value": "-2.39E-09", "module": "D", "scenario": "S2"}, {"value": "-7.02E-11", "module": "D", "scenario": "S3"}]}, "resolvedFlowVersion": "38.00.000", "flowProperties": [], "typeOfFlow": "Other flow", "classification": {"classHierarchy": "Quantities / Environmental quantities / EPD EN 15804 / LCI indicators", "name": "GaBiCategories"}}, {"dataSetInternalID": 12, "referenceToFlowDataSet": {"shortDescription": [{"value": "Non hazardous waste disposed (NHWD)", "lang": "en"}, {"value": "Entsorgter nicht gefährlicher Abfall (NHWD)", "lang": "de"}], "type": "flow data set", "refObjectId": "b29ef66b-e286-4afa-949f-62f1a7b4d7fa", "uri": "../flows/b29ef66b-e286-4afa-949f-62f1a7b4d7fa.xml"}, "exchange direction": "OUTPUT", "other": {"anies": [{"name": "referenceToUnitGroupDataSet", "value": {"shortDescription": [{"value": "kg", "lang": "en"}], "type": "unit group data set", "refObjectId": "ad38d542-3fe9-439d-9b95-2f5f7752acaf", "uri": "../unitgroups/ad38d542-3fe9-439d-9b95-2f5f7752acaf.xml"}}, {"value": "0.119", "module": "A1-A3"}, {"value": "0.000475", "module": "A4"}, {"value": "0.04017", "module": "A5"}, {"value": "0", "module": "B1"}, {"value": "0.0073", "module": "B2"}, {"value": "0", "module": "C1"}, {"value": "2.63E-05", "module": "C2"}, {"value": "1.21", "module": "C3", "scenario": "S2"}, {"value": "1.21", "module": "C3", "scenario": "S3"}, {"value": "4.03", "module": "C4"}, {"value": "-0.000385", "module": "D"}, {"value": "0", "module": "D", "scenario": "S1"}, {"value": "-0.00892", "module": "D", "scenario": "S2"}, {"value": "-0.000789", "module": "D", "scenario": "S3"}]}, "resolvedFlowVersion": "38.00.000", "flowProperties": [], "typeOfFlow": "Other flow", "classification": {"classHierarchy": "Quantities / Environmental quantities / EPD EN 15804 / LCI indicators", "name": "GaBiCategories"}}, {"dataSetInternalID": 13, "referenceToFlowDataSet": {"shortDescription": [{"value": "Radioactive waste disposed (RWD)", "lang": "en"}, {"value": "Entsorgter radioaktiver Abfall (RWD)", "lang": "de"}], "type": "flow data set", "refObjectId": "3449546e-52ad-4b39-b809-9fb77cea8ff6", "uri": "../flows/3449546e-52ad-4b39-b809-9fb77cea8ff6.xml"}, "exchange direction": "OUTPUT", "other": {"anies": [{"name": "referenceToUnitGroupDataSet", "value": {"shortDescription": [{"value": "kg", "lang": "en"}], "type": "unit group data set", "refObjectId": "ad38d542-3fe9-439d-9b95-2f5f7752acaf", "uri": "../unitgroups/ad38d542-3fe9-439d-9b95-2f5f7752acaf.xml"}}, {"value": "0.00413", "module": "A1-A3"}, {"value": "4.08E-06", "module": "A4"}, {"value": "0.00012732", "module": "A5"}, {"value": "0", "module": "B1"}, {"value": "0.000376", "module": "B2"}, {"value": "0", "module": "C1"}, {"value": "2.26E-07", "module": "C2"}, {"value": "0.000103", "module": "C3", "scenario": "S2"}, {"value": "0.000164", "module": "C3", "scenario": "S3"}, {"value": "5E-05", "module": "C4"}, {"value": "-5.99E-05", "module": "D"}, {"value": "0", "module": "D", "scenario": "S1"}, {"value": "-0.00139", "module": "D", "scenario": "S2"}, {"value": "-5.59E-05", "module": "D", "scenario": "S3"}]}, "resolvedFlowVersion": "38.00.000", "flowProperties": [], "typeOfFlow": "Other flow", "classification": {"classHierarchy": "Quantities / Environmental quantities / EPD EN 15804 / LCI indicators", "name": "GaBiCategories"}}, {"dataSetInternalID": 14, "referenceToFlowDataSet": {"shortDescription": [{"value": "Components for re-use (CRU)", "lang": "en"}, {"value": "Komponenten für die Wiederverwendung (CRU)", "lang": "de"}], "type": "flow data set", "refObjectId": "a2b32f97-3fc7-4af2-b209-525bc6426f33", "uri": "../flows/a2b32f97-3fc7-4af2-b209-525bc6426f33.xml"}, "exchange direction": "OUTPUT", "other": {"anies": [{"name": "referenceToUnitGroupDataSet", "value": {"shortDescription": [{"value": "kg", "lang": "en"}], "type": "unit group data set", "refObjectId": "ad38d542-3fe9-439d-9b95-2f5f7752acaf", "uri": "../unitgroups/ad38d542-3fe9-439d-9b95-2f5f7752acaf.xml"}}, {"value": "0", "module": "A1-A3"}, {"value": "0", "module": "A4"}, {"value": "0", "module": "A5"}, {"value": "0", "module": "B1"}, {"value": "0", "module": "B2"}, {"value": "0", "module": "C1"}, {"value": "0", "module": "C2"}, {"value": "0", "module": "C3", "scenario": "S2"}, {"value": "0", "module": "C3", "scenario": "S3"}, {"value": "0", "module": "C4"}, {"value": "0", "module": "D"}, {"value": "0", "module": "D", "scenario": "S1"}, {"value": "0", "module": "D", "scenario": "S2"}, {"value": "0", "module": "D", "scenario": "S3"}]}, "resolvedFlowVersion": "38.00.000", "flowProperties": [], "typeOfFlow": "Other flow", "classification": {"classHierarchy": "Quantities / Environmental quantities / EPD EN 15804 / LCI indicators", "name": "GaBiCategories"}}, {"dataSetInternalID": 15, "referenceToFlowDataSet": {"shortDescription": [{"value": "Materials for recycling (MFR)", "lang": "en"}, {"value": "Stoffe zum Recycling (MFR)", "lang": "de"}], "type": "flow data set", "refObjectId": "d7fe48a5-4103-49c8-9aae-b0b5dfdbd6ae", "uri": "../flows/d7fe48a5-4103-49c8-9aae-b0b5dfdbd6ae.xml"}, "exchange direction": "OUTPUT", "other": {"anies": [{"name": "referenceToUnitGroupDataSet", "value": {"shortDescription": [{"value": "kg", "lang": "en"}], "type": "unit group data set", "refObjectId": "ad38d542-3fe9-439d-9b95-2f5f7752acaf", "uri": "../unitgroups/ad38d542-3fe9-439d-9b95-2f5f7752acaf.xml"}}, {"value": "0", "module": "A1-A3"}, {"value": "0", "module": "A4"}, {"value": "0.121", "module": "A5"}, {"value": "0", "module": "B1"}, {"value": "0", "module": "B2"}, {"value": "0", "module": "C1"}, {"value": "0", "module": "C2"}, {"value": "0", "module": "C3", "scenario": "S2"}, {"value": "1.37", "module": "C3", "scenario": "S3"}, {"value": "0", "module": "C4"}, {"value": "0", "module": "D"}, {"value": "0", "module": "D", "scenario": "S1"}, {"value": "0", "module": "D", "scenario": "S2"}, {"value": "0", "module": "D", "scenario": "S3"}]}, "resolvedFlowVersion": "38.00.000", "flowProperties": [], "typeOfFlow": "Other flow", "classification": {"classHierarchy": "Quantities / Environmental quantities / EPD EN 15804 / LCI indicators", "name": "GaBiCategories"}}, {"dataSetInternalID": 16, "referenceToFlowDataSet": {"shortDescription": [{"value": "Materials for energy recovery (MER)", "lang": "en"}, {"value": "Stoffe für die Energierückgewinnung (MER)", "lang": "de"}], "type": "flow data set", "refObjectId": "59a9181c-3aaf-46ee-8b13-2b3723b6e447", "uri": "../flows/59a9181c-3aaf-46ee-8b13-2b3723b6e447.xml"}, "exchange direction": "OUTPUT", "other": {"anies": [{"name": "referenceToUnitGroupDataSet", "value": {"shortDescription": [{"value": "kg", "lang": "en"}], "type": "unit group data set", "refObjectId": "ad38d542-3fe9-439d-9b95-2f5f7752acaf", "uri": "../unitgroups/ad38d542-3fe9-439d-9b95-2f5f7752acaf.xml"}}, {"value": "0", "module": "A1-A3"}, {"value": "0", "module": "A4"}, {"value": "0", "module": "A5"}, {"value": "0", "module": "B1"}, {"value": "0", "module": "B2"}, {"value": "0", "module": "C1"}, {"value": "0", "module": "C2"}, {"value": "0", "module": "C3", "scenario": "S2"}, {"value": "0", "module": "C3", "scenario": "S3"}, {"value": "0", "module": "C4"}, {"value": "0", "module": "D"}, {"value": "0", "module": "D", "scenario": "S1"}, {"value": "0", "module": "D", "scenario": "S2"}, {"value": "0", "module": "D", "scenario": "S3"}]}, "resolvedFlowVersion": "38.00.000", "flowProperties": [], "typeOfFlow": "Other flow", "classification": {"classHierarchy": "Quantities / Environmental quantities / EPD EN 15804 / LCI indicators", "name": "GaBiCategories"}}, {"dataSetInternalID": 17, "referenceToFlowDataSet": {"shortDescription": [{"value": "Exported electrical energy (EEE)", "lang": "en"}, {"value": "Exportierte elektrische Energie (EEE)", "lang": "de"}], "type": "flow data set", "refObjectId": "4da0c987-2b76-40d6-9e9e-82a017aaaf29", "uri": "../flows/4da0c987-2b76-40d6-9e9e-82a017aaaf29.xml"}, "exchange direction": "OUTPUT", "other": {"anies": [{"name": "referenceToUnitGroupDataSet", "value": {"shortDescription": [{"value": "MJ", "lang": "en"}], "type": "unit group data set", "refObjectId": "93a60a57-a3c8-11da-a746-0800200c9a66", "uri": "../unitgroups/93a60a57-a3c8-11da-a746-0800200c9a66.xml"}}, {"value": "0", "module": "A1-A3"}, {"value": "0", "module": "A4"}, {"value": "0.187", "module": "A5"}, {"value": "0", "module": "B1"}, {"value": "0", "module": "B2"}, {"value": "0", "module": "C1"}, {"value": "0", "module": "C2"}, {"value": "4.17", "module": "C3", "scenario": "S2"}, {"value": "0", "module": "C3", "scenario": "S3"}, {"value": "0", "module": "C4"}, {"value": "0", "module": "D"}, {"value": "0", "module": "D", "scenario": "S1"}, {"value": "0", "module": "D", "scenario": "S2"}, {"value": "0", "module": "D", "scenario": "S3"}]}, "resolvedFlowVersion": "38.00.000", "flowProperties": [], "typeOfFlow": "Other flow", "classification": {"classHierarchy": "Quantities / Environmental quantities / EPD EN 15804 / LCI indicators", "name": "GaBiCategories"}}, {"dataSetInternalID": 18, "referenceToFlowDataSet": {"shortDescription": [{"value": "Exported thermal energy (EET)", "lang": "en"}, {"value": "Exportierte thermische Energie (EET)", "lang": "de"}], "type": "flow data set", "refObjectId": "98daf38a-7a79-46d3-9a37-2b7bd0955810", "uri": "../flows/98daf38a-7a79-46d3-9a37-2b7bd0955810.xml"}, "exchange direction": "OUTPUT", "other": {"anies": [{"name": "referenceToUnitGroupDataSet", "value": {"shortDescription": [{"value": "MJ", "lang": "en"}], "type": "unit group data set", "refObjectId": "93a60a57-a3c8-11da-a746-0800200c9a66", "uri": "../unitgroups/93a60a57-a3c8-11da-a746-0800200c9a66.xml"}}, {"value": "0", "module": "A1-A3"}, {"value": "0", "module": "A4"}, {"value": "0.349", "module": "A5"}, {"value": "0", "module": "B1"}, {"value": "0", "module": "B2"}, {"value": "0", "module": "C1"}, {"value": "0", "module": "C2"}, {"value": "8", "module": "C3", "scenario": "S2"}, {"value": "48.4", "module": "C3", "scenario": "S3"}, {"value": "0", "module": "C4"}, {"value": "0", "module": "D"}, {"value": "0", "module": "D", "scenario": "S1"}, {"value": "0", "module": "D", "scenario": "S2"}, {"value": "0", "module": "D", "scenario": "S3"}]}, "resolvedFlowVersion": "38.00.000", "flowProperties": [], "typeOfFlow": "Other flow", "classification": {"classHierarchy": "Quantities / Environmental quantities / EPD EN 15804 / LCI indicators", "name": "GaBiCategories"}}]}, "LCIAResults": {"LCIAResult": [{"referenceToLCIAMethodDataSet": {"shortDescription": [{"value": "Global Warming Potential total (GWP-total)", "lang": "en"}, {"value": "Globales Erwärmungspotenzial total (GWP-total)", "lang": "de"}], "type": "LCIA method data set", "refObjectId": "6a37f984-a4b3-458a-a20a-64418c145fa2", "uri": "../lciamethods/6a37f984-a4b3-458a-a20a-64418c145fa2.xml"}, "other": {"anies": [{"name": "referenceToUnitGroupDataSet", "value": {"shortDescription": [{"value": "kg CO_(2) eq", "lang": "en"}], "type": "unit group data set", "refObjectId": "1ebf3012-d0db-4de2-aefd-ef30cedb0be1", "uri": "../unitgroups/1ebf3012-d0db-4de2-aefd-ef30cedb0be1.xml"}}, {"value": "6.108", "module": "A1-A3"}, {"value": "0.248", "module": "A4"}, {"value": "0.37634", "module": "A5"}, {"value": "0", "module": "B1"}, {"value": "0.5488", "module": "B2"}, {"value": "0", "module": "C1"}, {"value": "0.01373", "module": "C2"}, {"value": "4.307", "module": "C3", "scenario": "S2"}, {"value": "4.362", "module": "C3", "scenario": "S3"}, {"value": "2.496", "module": "C4"}, {"value": "-0.04498", "module": "D"}, {"value": "0", "module": "D", "scenario": "S1"}, {"value": "-1.044", "module": "D", "scenario": "S2"}, {"value": "-0.2524", "module": "D", "scenario": "S3"}]}}, {"referenceToLCIAMethodDataSet": {"shortDescription": [{"value": "Global Warming Potential fossil fuels (GWP-fossil)", "lang": "en"}, {"value": "Globales Erwärmungspotenzial fossil (GWP-fossil)", "lang": "de"}], "type": "LCIA method data set", "refObjectId": "5f635281-343e-44fb-83df-1971b155e6b6", "uri": "../lciamethods/5f635281-343e-44fb-83df-1971b155e6b6.xml"}, "other": {"anies": [{"name": "referenceToUnitGroupDataSet", "value": {"shortDescription": [{"value": "kg CO_(2) eq", "lang": "en"}], "type": "unit group data set", "refObjectId": "1ebf3012-d0db-4de2-aefd-ef30cedb0be1", "uri": "../unitgroups/1ebf3012-d0db-4de2-aefd-ef30cedb0be1.xml"}}, {"value": "7.384", "module": "A1-A3"}, {"value": "0.2435", "module": "A4"}, {"value": "0.35422", "module": "A5"}, {"value": "0", "module": "B1"}, {"value": "0.3484", "module": "B2"}, {"value": "0", "module": "C1"}, {"value": "0.01348", "module": "C2"}, {"value": "3.2", "module": "C3", "scenario": "S2"}, {"value": "3.254", "module": "C3", "scenario": "S3"}, {"value": "1.3896", "module": "C4"}, {"value": "-0.04475", "module": "D"}, {"value": "0", "module": "D", "scenario": "S1"}, {"value": "-1.039", "module": "D", "scenario": "S2"}, {"value": "-0.252", "module": "D", "scenario": "S3"}]}}, {"referenceToLCIAMethodDataSet": {"shortDescription": [{"value": "Global Warming Potential biogenic (GWP-biogenic)", "lang": "en"}, {"value": "Globales Erwärmungspotenzial biogen (GWP-biogenic)", "lang": "de"}], "type": "LCIA method data set", "refObjectId": "2356e1ab-0185-4db5-86e5-16de51c7485c", "uri": "../lciamethods/2356e1ab-0185-4db5-86e5-16de51c7485c.xml"}, "other": {"anies": [{"name": "referenceToUnitGroupDataSet", "value": {"shortDescription": [{"value": "kg CO_(2) eq", "lang": "en"}], "type": "unit group data set", "refObjectId": "1ebf3012-d0db-4de2-aefd-ef30cedb0be1", "uri": "../unitgroups/1ebf3012-d0db-4de2-aefd-ef30cedb0be1.xml"}}, {"value": "-1.281", "module": "A1-A3"}, {"value": "0.003151", "module": "A4"}, {"value": "0.02187", "module": "A5"}, {"value": "0", "module": "B1"}, {"value": "0.004159", "module": "B2"}, {"value": "0", "module": "C1"}, {"value": "0.0001744", "module": "C2"}, {"value": "1.107", "module": "C3", "scenario": "S2"}, {"value": "1.107", "module": "C3", "scenario": "S3"}, {"value": "1.106", "module": "C4"}, {"value": "-0.0002289", "module": "D"}, {"value": "0", "module": "D", "scenario": "S1"}, {"value": "-0.005305", "module": "D", "scenario": "S2"}, {"value": "-0.0002846", "module": "D", "scenario": "S3"}]}}, {"referenceToLCIAMethodDataSet": {"shortDescription": [{"value": "Global Warming Potential luluc (GWP-luluc)", "lang": "en"}, {"value": "Globales Erwärmungspotenzial luluc (GWP-luluc)", "lang": "de"}], "type": "LCIA method data set", "refObjectId": "4331bbdb-978a-490d-8707-eeb047f01a55", "uri": "../lciamethods/4331bbdb-978a-490d-8707-eeb047f01a55.xml"}, "other": {"anies": [{"name": "referenceToUnitGroupDataSet", "value": {"shortDescription": [{"value": "kg CO_(2) eq", "lang": "en"}], "type": "unit group data set", "refObjectId": "1ebf3012-d0db-4de2-aefd-ef30cedb0be1", "uri": "../unitgroups/1ebf3012-d0db-4de2-aefd-ef30cedb0be1.xml"}}, {"value": "0.004477", "module": "A1-A3"}, {"value": "0.001379", "module": "A4"}, {"value": "0.00018649", "module": "A5"}, {"value": "0", "module": "B1"}, {"value": "0.1962", "module": "B2"}, {"value": "0", "module": "C1"}, {"value": "7.633E-05", "module": "C2"}, {"value": "0.0002464", "module": "C3", "scenario": "S2"}, {"value": "0.0004416", "module": "C3", "scenario": "S3"}, {"value": "0.0001396", "module": "C4"}, {"value": "-4.919E-06", "module": "D"}, {"value": "0", "module": "D", "scenario": "S1"}, {"value": "-0.000114", "module": "D", "scenario": "S2"}, {"value": "-0.0001053", "module": "D", "scenario": "S3"}]}}, {"referenceToLCIAMethodDataSet": {"shortDescription": [{"value": "Depletion potential of the stratospheric ozone layer (ODP)", "lang": "en"}, {"value": "Abbau Potential der stratosphärischen Ozonschicht (ODP)", "lang": "de"}], "type": "LCIA method data set", "refObjectId": "b5c629d6-def3-11e6-bf01-fe55135034f3", "uri": "../lciamethods/b5c629d6-def3-11e6-bf01-fe55135034f3.xml"}, "other": {"anies": [{"name": "referenceToUnitGroupDataSet", "value": {"shortDescription": [{"value": "kg CFC11 eq", "lang": "en"}], "type": "unit group data set", "refObjectId": "d9e957c9-7309-4474-bf3a-7777df6c4e5b", "uri": "../unitgroups/d9e957c9-7309-4474-bf3a-7777df6c4e5b.xml"}}, {"value": "1.368E-08", "module": "A1-A3"}, {"value": "1.482E-14", "module": "A4"}, {"value": "4.104108E-10", "module": "A5"}, {"value": "0", "module": "B1"}, {"value": "3.415E-08", "module": "B2"}, {"value": "0", "module": "C1"}, {"value": "8.202E-16", "module": "C2"}, {"value": "3.028E-13", "module": "C3", "scenario": "S2"}, {"value": "6.082E-13", "module": "C3", "scenario": "S3"}, {"value": "3.851E-13", "module": "C4"}, {"value": "-3.026E-13", "module": "D"}, {"value": "0", "module": "D", "scenario": "S1"}, {"value": "-7.006E-12", "module": "D", "scenario": "S2"}, {"value": "-4.669E-13", "module": "D", "scenario": "S3"}]}}, {"referenceToLCIAMethodDataSet": {"shortDescription": [{"value": "Acidification potential of land and water (AP)", "lang": "en"}, {"value": "Versauerungspotenzial von Boden und Wasser (AP)", "lang": "de"}], "type": "LCIA method data set", "refObjectId": "b5c611c6-def3-11e6-bf01-fe55135034f3", "uri": "../lciamethods/b5c611c6-def3-11e6-bf01-fe55135034f3.xml"}, "other": {"anies": [{"name": "referenceToUnitGroupDataSet", "value": {"shortDescription": [{"value": "mol H^(+) eq", "lang": "en"}], "type": "unit group data set", "refObjectId": "42e089ac-92bf-4bf2-8ca1-5fc40d18f2ed", "uri": "../unitgroups/42e089ac-92bf-4bf2-8ca1-5fc40d18f2ed.xml"}}, {"value": "0.01526", "module": "A1-A3"}, {"value": "0.001472", "module": "A4"}, {"value": "0.0005842", "module": "A5"}, {"value": "0", "module": "B1"}, {"value": "0.000832", "module": "B2"}, {"value": "0", "module": "C1"}, {"value": "8.151E-05", "module": "C2"}, {"value": "0.002523", "module": "C3", "scenario": "S2"}, {"value": "0.002773", "module": "C3", "scenario": "S3"}, {"value": "0.0008497", "module": "C4"}, {"value": "-5.887E-05", "module": "D"}, {"value": "0", "module": "D", "scenario": "S1"}, {"value": "-0.001364", "module": "D", "scenario": "S2"}, {"value": "-0.00073", "module": "D", "scenario": "S3"}]}}, {"referenceToLCIAMethodDataSet": {"shortDescription": [{"value": "Eutrophication potential aquatic freshwater (EP-freshwater)", "lang": "en"}, {"value": "Eutrophierungspotenzial Süßwasser (EP-freshwater)", "lang": "de"}], "type": "LCIA method data set", "refObjectId": "b53ec18f-7377-4ad3-86eb-cc3f4f276b2b", "uri": "../lciamethods/b53ec18f-7377-4ad3-86eb-cc3f4f276b2b.xml"}, "other": {"anies": [{"name": "referenceToUnitGroupDataSet", "value": {"shortDescription": [{"value": "kg P eq", "lang": "en"}], "type": "unit group data set", "refObjectId": "0429039d-a61d-4590-ba67-aa4a20a810a1", "uri": "../unitgroups/0429039d-a61d-4590-ba67-aa4a20a810a1.xml"}}, {"value": "0.000109", "module": "A1-A3"}, {"value": "7.382E-07", "module": "A4"}, {"value": "3.31948E-06", "module": "A5"}, {"value": "0", "module": "B1"}, {"value": "5.189E-06", "module": "B2"}, {"value": "0", "module": "C1"}, {"value": "4.087E-08", "module": "C2"}, {"value": "8.41E-07", "module": "C3", "scenario": "S2"}, {"value": "1.004E-06", "module": "C3", "scenario": "S3"}, {"value": "5.352E-05", "module": "C4"}, {"value": "-6.157E-08", "module": "D"}, {"value": "0", "module": "D", "scenario": "S1"}, {"value": "-1.426E-06", "module": "D", "scenario": "S2"}, {"value": "-2.492E-07", "module": "D", "scenario": "S3"}]}}, {"referenceToLCIAMethodDataSet": {"shortDescription": [{"value": "Eutrophication potential aquatic marine (EP-marine)", "lang": "en"}, {"value": "Eutrophierungspotenzial Salzwasser (EP-marine)", "lang": "de"}], "type": "LCIA method data set", "refObjectId": "b5c619fa-def3-11e6-bf01-fe55135034f3", "uri": "../lciamethods/b5c619fa-def3-11e6-bf01-fe55135034f3.xml"}, "other": {"anies": [{"name": "referenceToUnitGroupDataSet", "value": {"shortDescription": [{"value": "kg N eq", "lang": "en"}], "type": "unit group data set", "refObjectId": "d05bb823-ecdf-4686-8c40-bf1d9257859f", "uri": "../unitgroups/d05bb823-ecdf-4686-8c40-bf1d9257859f.xml"}}, {"value": "0.004389", "module": "A1-A3"}, {"value": "0.0007228", "module": "A4"}, {"value": "0.00019048", "module": "A5"}, {"value": "0", "module": "B1"}, {"value": "0.000197", "module": "B2"}, {"value": "0", "module": "C1"}, {"value": "4.002E-05", "module": "C2"}, {"value": "0.001158", "module": "C3", "scenario": "S2"}, {"value": "0.001269", "module": "C3", "scenario": "S3"}, {"value": "0.000188", "module": "C4"}, {"value": "-1.597E-05", "module": "D"}, {"value": "0", "module": "D", "scenario": "S1"}, {"value": "-0.0003704", "module": "D", "scenario": "S2"}, {"value": "-0.0002476", "module": "D", "scenario": "S3"}]}}, {"referenceToLCIAMethodDataSet": {"shortDescription": [{"value": "Eutrophication potential terrestrial (EP-terrestrial)", "lang": "en"}, {"value": "Eutrophierungspotenzial Land (EP-terrestrial)", "lang": "de"}], "type": "LCIA method data set", "refObjectId": "b5c614d2-def3-11e6-bf01-fe55135034f3", "uri": "../lciamethods/b5c614d2-def3-11e6-bf01-fe55135034f3.xml"}, "other": {"anies": [{"name": "referenceToUnitGroupDataSet", "value": {"shortDescription": [{"value": "mol N eq", "lang": "en"}], "type": "unit group data set", "refObjectId": "71b4d617-0ec9-4d3f-b65e-e438940c2401", "uri": "../unitgroups/71b4d617-0ec9-4d3f-b65e-e438940c2401.xml"}}, {"value": "0.04273", "module": "A1-A3"}, {"value": "0.008001", "module": "A4"}, {"value": "0.0019473", "module": "A5"}, {"value": "0", "module": "B1"}, {"value": "0.002831", "module": "B2"}, {"value": "0", "module": "C1"}, {"value": "0.0004429", "module": "C2"}, {"value": "0.01308", "module": "C3", "scenario": "S2"}, {"value": "0.01429", "module": "C3", "scenario": "S3"}, {"value": "0.002062", "module": "C4"}, {"value": "-0.000171", "module": "D"}, {"value": "0", "module": "D", "scenario": "S1"}, {"value": "-0.003967", "module": "D", "scenario": "S2"}, {"value": "-0.002713", "module": "D", "scenario": "S3"}]}}, {"referenceToLCIAMethodDataSet": {"shortDescription": [{"value": "Formation potential of tropospheric ozone photochemical oxidants (POCP)", "lang": "en"}, {"value": "Bildungspotential für troposphärisches Ozon (POCP)", "lang": "de"}], "type": "LCIA method data set", "refObjectId": "b5c610fe-def3-11e6-bf01-fe55135034f3", "uri": "../lciamethods/b5c610fe-def3-11e6-bf01-fe55135034f3.xml"}, "other": {"anies": [{"name": "referenceToUnitGroupDataSet", "value": {"shortDescription": [{"value": "kg NMVOC eq", "lang": "en"}], "type": "unit group data set", "refObjectId": "d27c25f8-fbc1-44c6-b47b-4adbae4199c6", "uri": "../unitgroups/d27c25f8-fbc1-44c6-b47b-4adbae4199c6.xml"}}, {"value": "0.01313", "module": "A1-A3"}, {"value": "0.001366", "module": "A4"}, {"value": "0.0005299", "module": "A5"}, {"value": "0.000418", "module": "B1"}, {"value": "0.0009833", "module": "B2"}, {"value": "0", "module": "C1"}, {"value": "7.565E-05", "module": "C2"}, {"value": "0.002996", "module": "C3", "scenario": "S2"}, {"value": "0.003213", "module": "C3", "scenario": "S3"}, {"value": "0.0006047", "module": "C4"}, {"value": "-4.469E-05", "module": "D"}, {"value": "0", "module": "D", "scenario": "S1"}, {"value": "-0.001037", "module": "D", "scenario": "S2"}, {"value": "-0.000769", "module": "D", "scenario": "S3"}]}}, {"referenceToLCIAMethodDataSet": {"shortDescription": [{"value": "Abiotic depletion potential for non fossil resources (ADPE)", "lang": "en"}, {"value": "Potenzial für den abiotischen Abbau nicht fossiler Ressourcen (ADPE)", "lang": "de"}], "type": "LCIA method data set", "refObjectId": "b2ad6494-c78d-11e6-9d9d-cec0c932ce01", "uri": "../lciamethods/b2ad6494-c78d-11e6-9d9d-cec0c932ce01.xml"}, "other": {"anies": [{"name": "referenceToUnitGroupDataSet", "value": {"shortDescription": [{"value": "kg Sb eq", "lang": "en"}], "type": "unit group data set", "refObjectId": "54ccd2d9-a32a-4fc2-923d-f2c8c93e89d4", "uri": "../unitgroups/54ccd2d9-a32a-4fc2-923d-f2c8c93e89d4.xml"}}, {"value": "2.191E-06", "module": "A1-A3"}, {"value": "2.067E-08", "module": "A4"}, {"value": "6.7119E-08", "module": "A5"}, {"value": "0", "module": "B1"}, {"value": "2.301E-07", "module": "B2"}, {"value": "0", "module": "C1"}, {"value": "1.145E-09", "module": "C2"}, {"value": "2.294E-08", "module": "C3", "scenario": "S2"}, {"value": "3.145E-08", "module": "C3", "scenario": "S3"}, {"value": "1.988E-08", "module": "C4"}, {"value": "-6.753E-09", "module": "D"}, {"value": "0", "module": "D", "scenario": "S1"}, {"value": "-1.565E-07", "module": "D", "scenario": "S2"}, {"value": "-2.25E-08", "module": "D", "scenario": "S3"}]}}, {"referenceToLCIAMethodDataSet": {"shortDescription": [{"value": "Abiotic depletion potential for fossil resources (ADPF)", "lang": "en"}, {"value": "Potenzial für den abiotischen Abbau fossiler Brennstoffe (ADPF)", "lang": "de"}], "type": "LCIA method data set", "refObjectId": "b2ad6110-c78d-11e6-9d9d-cec0c932ce01", "uri": "../lciamethods/b2ad6110-c78d-11e6-9d9d-cec0c932ce01.xml"}, "other": {"anies": [{"name": "referenceToUnitGroupDataSet", "value": {"shortDescription": [{"value": "MJ", "lang": "en"}], "type": "unit group data set", "refObjectId": "93a60a57-a3c8-11da-a746-0800200c9a66", "uri": "../unitgroups/93a60a57-a3c8-11da-a746-0800200c9a66.xml"}}, {"value": "159.9", "module": "A1-A3"}, {"value": "3.305", "module": "A4"}, {"value": "4.9846", "module": "A5"}, {"value": "0", "module": "B1"}, {"value": "5.897", "module": "B2"}, {"value": "0", "module": "C1"}, {"value": "0.183", "module": "C2"}, {"value": "2.565", "module": "C3", "scenario": "S2"}, {"value": "3.398", "module": "C3", "scenario": "S3"}, {"value": "4.068", "module": "C4"}, {"value": "-0.761", "module": "D"}, {"value": "0", "module": "D", "scenario": "S1"}, {"value": "-17.66", "module": "D", "scenario": "S2"}, {"value": "-40.89", "module": "D", "scenario": "S3"}]}}, {"referenceToLCIAMethodDataSet": {"shortDescription": [{"value": "Water use (WDP)", "lang": "en"}, {"value": "Wassernutzung (WDP)", "lang": "de"}], "type": "LCIA method data set", "refObjectId": "b2ad66ce-c78d-11e6-9d9d-cec0c932ce01", "uri": "../lciamethods/b2ad66ce-c78d-11e6-9d9d-cec0c932ce01.xml"}, "other": {"anies": [{"name": "referenceToUnitGroupDataSet", "value": {"shortDescription": [{"value": "m^(3) world eq deprived", "lang": "en"}], "type": "unit group data set", "refObjectId": "6ae2df01-888e-46c8-b17d-49fa3869b476", "uri": "../unitgroups/6ae2df01-888e-46c8-b17d-49fa3869b476.xml"}}, {"value": "14.84", "module": "A1-A3"}, {"value": "0.002212", "module": "A4"}, {"value": "0.46606", "module": "A5"}, {"value": "0", "module": "B1"}, {"value": "0.09986", "module": "B2"}, {"value": "0", "module": "C1"}, {"value": "0.0001224", "module": "C2"}, {"value": "0.6045", "module": "C3", "scenario": "S2"}, {"value": "0.6095", "module": "C3", "scenario": "S3"}, {"value": "-0.003042", "module": "C4"}, {"value": "-0.004716", "module": "D"}, {"value": "0", "module": "D", "scenario": "S1"}, {"value": "-0.1092", "module": "D", "scenario": "S2"}, {"value": "-0.04088", "module": "D", "scenario": "S3"}]}}, {"referenceToLCIAMethodDataSet": {"shortDescription": [{"value": "Incidence of disease due to PM emissions (PM)", "lang": "en"}, {"value": "Auftreten von Krankheiten aufgrund von Feinstaubemissionen (PM)", "lang": "de"}], "type": "LCIA method data set", "refObjectId": "b5c602c6-def3-11e6-bf01-fe55135034f3", "uri": "../lciamethods/b5c602c6-def3-11e6-bf01-fe55135034f3.xml"}, "other": {"anies": [{"name": "referenceToUnitGroupDataSet", "value": {"shortDescription": [{"value": "Disease incidence", "lang": "en"}], "type": "unit group data set", "refObjectId": "3883559b-648f-4afc-8ba2-0bd24f3affa3", "uri": "../unitgroups/3883559b-648f-4afc-8ba2-0bd24f3affa3.xml"}}, {"value": "1.22E-07", "module": "A1-A3"}, {"value": "8.51E-09", "module": "A4"}, {"value": "4.488E-09", "module": "A5"}, {"value": "0", "module": "B1"}, {"value": "6.84E-08", "module": "B2"}, {"value": "0", "module": "C1"}, {"value": "4.71E-10", "module": "C2"}, {"value": "1.78E-08", "module": "C3", "scenario": "S2"}, {"value": "1.94E-08", "module": "C3", "scenario": "S3"}, {"value": "8.17E-09", "module": "C4"}, {"value": "-4.88E-10", "module": "D"}, {"value": "0", "module": "D", "scenario": "S1"}, {"value": "0", "module": "D", "scenario": "S2"}, {"value": "-9.52E-09", "module": "D", "scenario": "S3"}]}}, {"referenceToLCIAMethodDataSet": {"shortDescription": [{"value": "Human exposure efficiency relative to U235 (IR)", "lang": "en"}, {"value": "Wirkung durch Exposition des Menschen mit U235 (IR)", "lang": "de"}], "type": "LCIA method data set", "refObjectId": "b5c632be-def3-11e6-bf01-fe55135034f3", "uri": "../lciamethods/b5c632be-def3-11e6-bf01-fe55135034f3.xml"}, "other": {"anies": [{"name": "referenceToUnitGroupDataSet", "value": {"shortDescription": [{"value": "kBq U235 eq", "lang": "en"}], "type": "unit group data set", "refObjectId": "456b05bf-1415-44a9-9993-02452f554c09", "uri": "../unitgroups/456b05bf-1415-44a9-9993-02452f554c09.xml"}}, {"value": "0.662", "module": "A1-A3"}, {"value": "0.000598", "module": "A4"}, {"value": "0.020383", "module": "A5"}, {"value": "0", "module": "B1"}, {"value": "0.0678", "module": "B2"}, {"value": "0", "module": "C1"}, {"value": "3.31E-05", "module": "C2"}, {"value": "0.0157", "module": "C3", "scenario": "S2"}, {"value": "0.0259", "module": "C3", "scenario": "S3"}, {"value": "0.00738", "module": "C4"}, {"value": "-0.0102", "module": "D"}, {"value": "0", "module": "D", "scenario": "S1"}, {"value": "0", "module": "D", "scenario": "S2"}, {"value": "-0.00481", "module": "D", "scenario": "S3"}]}}, {"referenceToLCIAMethodDataSet": {"shortDescription": [{"value": "Comparative toxic unit for ecosystems (ETP-fw)", "lang": "en"}, {"value": "Toxizitätsvergleichseinheit für Ökosysteme (ETP-fw)", "lang": "de"}], "type": "LCIA method data set", "refObjectId": "ee1082d1-b0f7-43ca-a1f0-21e2a4a74511", "uri": "../lciamethods/ee1082d1-b0f7-43ca-a1f0-21e2a4a74511.xml"}, "other": {"anies": [{"name": "referenceToUnitGroupDataSet", "value": {"shortDescription": [{"value": "CTUe", "lang": "en"}], "type": "unit group data set", "refObjectId": "aa959ded-f1eb-4efb-9c5c-2d60be36b3e6", "uri": "../unitgroups/aa959ded-f1eb-4efb-9c5c-2d60be36b3e6.xml"}}, {"value": "117", "module": "A1-A3"}, {"value": "2.29", "module": "A4"}, {"value": "3.631", "module": "A5"}, {"value": "0.0036", "module": "B1"}, {"value": "2.69", "module": "B2"}, {"value": "0", "module": "C1"}, {"value": "0.127", "module": "C2"}, {"value": "1.49", "module": "C3", "scenario": "S2"}, {"value": "1.97", "module": "C3", "scenario": "S3"}, {"value": "3.98", "module": "C4"}, {"value": "-0.167", "module": "D"}, {"value": "0", "module": "D", "scenario": "S1"}, {"value": "0", "module": "D", "scenario": "S2"}, {"value": "-6.87", "module": "D", "scenario": "S3"}]}}, {"referenceToLCIAMethodDataSet": {"shortDescription": [{"value": "Comparative toxic unit for humans (carcinogenic) (HTP-c)", "lang": "en"}, {"value": "Toxizitätsvergleichseinheit für Menschen (krebserregend) (HTP-c)", "lang": "de"}], "type": "LCIA method data set", "refObjectId": "2299222a-bbd8-474f-9d4f-4dd1f18aea7c", "uri": "../lciamethods/2299222a-bbd8-474f-9d4f-4dd1f18aea7c.xml"}, "other": {"anies": [{"name": "referenceToUnitGroupDataSet", "value": {"shortDescription": [{"value": "CTUh", "lang": "en"}], "type": "unit group data set", "refObjectId": "d4c9523e-2d7e-49fd-8469-998f547d3a70", "uri": "../unitgroups/d4c9523e-2d7e-49fd-8469-998f547d3a70.xml"}}, {"value": "2.54E-09", "module": "A1-A3"}, {"value": "4.64E-11", "module": "A4"}, {"value": "7.994E-11", "module": "A5"}, {"value": "0", "module": "B1"}, {"value": "6.21E-10", "module": "B2"}, {"value": "0", "module": "C1"}, {"value": "2.57E-12", "module": "C2"}, {"value": "6.84E-11", "module": "C3", "scenario": "S2"}, {"value": "7.95E-11", "module": "C3", "scenario": "S3"}, {"value": "1.79E-10", "module": "C4"}, {"value": "-7.68E-12", "module": "D"}, {"value": "0", "module": "D", "scenario": "S1"}, {"value": "0", "module": "D", "scenario": "S2"}, {"value": "-6.07E-11", "module": "D", "scenario": "S3"}]}}, {"referenceToLCIAMethodDataSet": {"shortDescription": [{"value": "Comparative toxic unit for humans (noncarcinogenic) (HTP-nc)", "lang": "en"}, {"value": "Toxizitätsvergleichseinheit für Menschen (nicht krebserregend) (HTP-nc)", "lang": "de"}], "type": "LCIA method data set", "refObjectId": "3af763a5-b7a1-48c9-9cee-1f223481fcef", "uri": "../lciamethods/3af763a5-b7a1-48c9-9cee-1f223481fcef.xml"}, "other": {"anies": [{"name": "referenceToUnitGroupDataSet", "value": {"shortDescription": [{"value": "CTUh", "lang": "en"}], "type": "unit group data set", "refObjectId": "d4c9523e-2d7e-49fd-8469-998f547d3a70", "uri": "../unitgroups/d4c9523e-2d7e-49fd-8469-998f547d3a70.xml"}}, {"value": "1.03E-07", "module": "A1-A3"}, {"value": "2.75E-09", "module": "A4"}, {"value": "3.335E-09", "module": "A5"}, {"value": "2.6E-11", "module": "B1"}, {"value": "9.46E-09", "module": "B2"}, {"value": "0", "module": "C1"}, {"value": "1.52E-10", "module": "C2"}, {"value": "4.99E-09", "module": "C3", "scenario": "S2"}, {"value": "5.55E-09", "module": "C3", "scenario": "S3"}, {"value": "1.5E-08", "module": "C4"}, {"value": "-2.95E-10", "module": "D"}, {"value": "0", "module": "D", "scenario": "S1"}, {"value": "0", "module": "D", "scenario": "S2"}, {"value": "-3.07E-09", "module": "D", "scenario": "S3"}]}}, {"referenceToLCIAMethodDataSet": {"shortDescription": [{"value": "Soil quality index (SQP)", "lang": "en"}, {"value": "Bodenqualitätsindex (SQP)", "lang": "de"}], "type": "LCIA method data set", "refObjectId": "b2ad6890-c78d-11e6-9d9d-cec0c932ce01", "uri": "../lciamethods/b2ad6890-c78d-11e6-9d9d-cec0c932ce01.xml"}, "other": {"anies": [{"name": "referenceToUnitGroupDataSet", "value": {"shortDescription": [{"value": "SQP", "lang": "en"}], "type": "unit group data set", "refObjectId": "f130951c-e67f-4f7f-8dd4-665de3974e18", "uri": "../unitgroups/f130951c-e67f-4f7f-8dd4-665de3974e18.xml"}}, {"module": "A1-A3"}, {"module": "A4"}, {"module": "A5"}, {"module": "B1"}, {"module": "B2"}, {"module": "C1"}, {"module": "C2"}, {"module": "C3", "scenario": "S2"}, {"module": "C3", "scenario": "S3"}, {"module": "C4"}, {"module": "D"}, {"module": "D", "scenario": "S1"}, {"module": "D", "scenario": "S2"}, {"module": "D", "scenario": "S3"}]}}]}, "otherAttributes": {"{http://www.indata.network/EPD/2019}epd-version": "1.2"}, "version": "1.1", "locations": "../ILCDLocations.xml"}