{"processInformation": {"dataSetInformation": {"UUID": "7b06ebcb-bf35-4ce0-8562-04a31cc7a315", "name": {"baseName": [{"value": "Amorim Wise Cork Pure PU PF", "lang": "en"}, {"value": "Amorim Wise Cork Pure PU PF", "lang": "de"}], "functionalUnitFlowProperties": [{"lang": "en"}]}, "classificationInformation": {"classification": [{"class": [{"value": "Holz", "level": 0, "classId": "3"}, {"value": "Holzböden", "level": 1, "classId": "3.3"}, {"value": "Mehrschichtig modulare Bodenbeläge", "level": 2, "classId": "3.3.04"}], "name": "OEKOBAU.DAT"}, {"class": [{"value": "02 Building products", "level": 0}, {"value": "Floor coverings", "level": 1}, {"value": "Floor coverings", "level": 2}], "name": "IBUCategories"}]}, "generalComment": [{"value": "Amorim Wise Cork Pure Polyurethane Prefinished (hereby referred to as Cork Pure PU PF) has a natural cork structure, that provides superior comfort and environmental performance for residential areas, with a genuine cork veneer decorative layer and polyurethane finishing. This product is used as a floor covering for domestic use, providing several physical characteristics to the floor, such as stability, comfort, thermal and noise insulation, among others.", "lang": "en"}], "other": {"anies": [{"scenario": [{"description": [{"value": "100% Incineration (C3/1, D/1)", "lang": "en"}, {"value": "100 % Verbrennung (C3/1, D/1)", "lang": "de"}], "name": "S1"}, {"description": [{"value": "100% Landfill (C4/2, D/2)", "lang": "en"}, {"value": "100 % Deponie (C4/2, D/2)", "lang": "de"}], "name": "S2"}]}]}}, "quantitativeReference": {"referenceToReferenceFlow": [0]}, "time": {"referenceYear": 2022, "dataSetValidUntil": 2027, "other": {"anies": [{"name": "publicationDateOfEPD", "value": 1670371200000}]}}, "geography": {"locationOfOperationSupplyOrProduction": {"location": "PT"}}, "technology": {"technologyDescriptionAndIncludedProcesses": [{"value": "The manufacturing process of Amorim Wise Cork Pure PU PF begins with cork granulate production, using cork that was previously treated at Amorim Florestal. Around 88% of the granulated cork previously produced is forwarded to an agglomeration process in which a melamine-urea-formaldehyde (MUF) resin is used to produce the agglomerated cork layer. This layer is the inferior layer of the final product and constitutes most of the thickness of the product. The remaining granulated cork, together with a polyvinyl acetate (PVA) resin, is used to produce the genuine cork veener, the decorative layer of the Amorim Wise Cork Pure PU PF. The agglomerated cork layer and the decorative genuine cork veener, that compose the final product structure are glued together using glue and adhesives as binding agents. This unfinished product then follows to a pressure and heat process, before going through sanding. The product is ultimately varnished with a base coat as well as a top coat varnish finishing of Polyurethane and forwarded for the final cut of the pieces. The top coat varnishing finalize the product in this stage of the Amorim Wise Cork Pure PU PF product, which is then packed and stored in the shipment warehouse, ready for shipment. \nTechnical data: \nRelevant technical construction data for the product is referred in the following table. \nDeclared unit: \nThe declared unit is 1 m2 of installed floor covering with the following characteristics:", "lang": "en"}, {"value": "Der Herstellungsprozess von Amorim Wise Cork Pure PU PF beginnt mit der Herstellung von Korkgranulat, wobei Kork verwendet wird, der zuvor bei Amorim Florestal behandelt wurde.\n\nRund 88 % des zuvor hergestellten Korkgranulats werden einem Agglomerationsprozess zugeführt, bei dem ein Melamin-Harnstoff-Formaldehyd-Harz (MUF) zur Herstellung der Agglomeratkorkschicht verwendet wird. Diese Schicht ist die untere Schicht des Endprodukts und macht den größten Teil der Dicke des Produkts aus. Das verbleibende Korkgranulat wird zusammen mit einem Polyvinylacetat (PVA)-Harz zur Herstellung des echten Korkfurniers, der dekorativen Schicht des Amorim Wise Cork Pure PU PF, verwendet.\n\nDie agglomerierte Korkschicht und das dekorative echte Korkfurnier, die die endgültige Produktstruktur bilden, werden unter Verwendung von Leim und Klebstoffen als Bindemittel miteinander verklebt. Dieses Rohprodukt wird dann einem Druck- und Wärmeprozess unterzogen, bevor es geschliffen wird.\n\nDas Produkt wird schließlich mit einem Basislack sowie einer Decklackierung aus Polyurethan lackiert und zum endgültigen Zuschnitt der Stücke weitergeleitet. Die Decklackierung stellt das Produkt in dieser Phase des Amorim Wise Cork Pure PU PF-Produkts fertig, das dann verpackt und versandfertig im Versandlager gelagert wird. \n", "lang": "de"}], "technologicalApplicability": [{"value": "Amorim Wise Cork Pure PU PF fits the most demanding needs for domestic areas. This flooring product meets the requirements of the usage class 23 for domestic use according to ISO 10874 standard.", "lang": "en"}, {"value": "Amorim Wise Cork Pure PU PF erfüllt die anspruchsvollsten Anforderungen im Wohnbereich. Dieses Bodenbelagsprodukt erfüllt die Anforderungen der Nutzungsklasse 23 für den Hausgebrauch gemäß der Norm ISO 10874.", "lang": "de"}]}}, "modellingAndValidation": {"LCIMethodAndAllocation": {"typeOfDataSet": "EPD", "referenceToLCAMethodDetails": [{"shortDescription": [{"value": "Floor coverings.pdf", "lang": "en"}], "type": "source data set", "refObjectId": "32406094-d79f-4884-9291-80f66b776484"}], "other": {"anies": [{"name": "subType", "value": "average dataset"}]}}, "dataSourcesTreatmentAndRepresentativeness": {"referenceToDataSource": [{"shortDescription": [{"value": "ecoinvent database (all versions)", "lang": "en"}], "type": "source data set", "refObjectId": "b497a91f-e14b-4b69-8f28-f50eb1576766"}, {"shortDescription": [{"value": "ecoinvent 3.5 database", "lang": "en"}], "type": "source data set", "refObjectId": "ca0da4f4-c837-4005-9c17-e77b9bd09d8b"}], "useAdviceForDataSet": [{"value": "Scope: \nThe data on which the Life Cycle Assessment is based is from the manufacturing process of Amorim Wise Cork Pure PU PF taking place in one industrial unit of Amorim Revestimentos (Oleiros) and is referred to the year of 2020. For the construction, use, end of life stages and benefits and loads, data were estimated based on background research and Amorim Cork Flooring supply chain downstream activities. Data associated with the product’s maintenance was obtained through benchmark research. \nSystem boundary: \nType of EPD: cradle to gate with options \n\n\nModules A1-A3 Production:  Include processes that provide materials, transport of the material to the manufacturing site, energy supply, product manufacturing and transport processes up to the factory gate, as well as waste processing. Biogenic carbon contained in the product and the packaging materials is included in this module. \n\n\nModule A4 Transport: Transport of the floor covering from the factory gate to the place of installation. \n\n\nModule A5 Installation: Includes material losses (offcuts) during the installation of the floor covering, use of adhesives and disposal of offcuts and recycling of packaging material. \n\n\nModule B2 Maintenance: includes provision of energy, for vacuum cleaning once a week, cleaning agent and water consumption, for wet cleaning twice a year. \n\nThe LCA results in this EPD are declared for a one-year usage. \n\n\nModule C1 De-construction: The floor covering is de-constructed manually and no additional environmental impact is caused. \n\n\nModule C2 Transport: Includes transportation of the postconsumer waste to the waste incineration plant or to a landfill \n\n\nModule C3 Waste processing and Module C4 Disposal, end-of-life scenarios are declared for: \n\n·         40 % incineration in a waste incineration plant (WIP) and 60 % landfilling (Mixed scenario) \n\n·         100 % incineration in a waste incineration plant (WIP) (Scenario 1) \n\n·         100 % landfilling (Scenario 2) \n\nModule D Benefits and Loads: Declares potential benefits from all net flows given in module A5 (packaging material recycling) and C3 (for incineration, and related energy substitution) that leave the product boundary system after having passed the end-of-waste state. Module D is declared for each scenario separately.", "lang": "en"}], "other": {"anies": [{"name": "referenceToOriginalEPD", "value": {"shortDescription": {"value": "Amorim Wise Cork Pure PU PF.pdf", "defaultValue": "Amorim Wise Cork Pure PU PF.pdf", "lstrings": [{"lang": "en", "value": "Amorim Wise Cork Pure PU PF.pdf"}]}, "type": "source data set", "uuid": {"uuid": "8d947849-a068-411c-b47a-3961d0f4b0cf"}, "refObjectId": "8d947849-a068-411c-b47a-3961d0f4b0cf", "resourceURLs": ["https://oekobaudat.de/OEKOBAU.DAT/resource/sources/8d947849-a068-411c-b47a-3961d0f4b0cf/Amorim_Wise_Cork_Pure_PU_PF_15110.pdf?version=00.01.000"]}}]}}, "validation": {"review": [{"referenceToNameOfReviewerAndInstitution": [{"shortDescription": [{"value": "Institut Bauen und Umwelt e. V.", "lang": "en"}], "type": "contact data set", "refObjectId": "d111dbec-b024-4be5-86c5-752d6eb2cf95", "uri": "../contacts/d111dbec-b024-4be5-86c5-752d6eb2cf95.xml"}], "type": "Accredited third party review"}]}, "complianceDeclarations": {"compliance": [{"referenceToComplianceSystem": {"shortDescription": [{"value": "DIN EN 15804+A2", "lang": "en"}], "type": "source data set", "refObjectId": "c0016b33-8cf7-415c-ac6e-deba0d21440d", "uri": "../sources/c0016b33-8cf7-415c-ac6e-deba0d21440d.xml"}}, {"referenceToComplianceSystem": {"shortDescription": [{"value": "ISO 14025", "lang": "en"}], "type": "source data set", "refObjectId": "4f2eb655-6e44-4874-a95a-e28f5442cd4d", "uri": "../sources/4f2eb655-6e44-4874-a95a-e28f5442cd4d.xml"}}]}}, "administrativeInformation": {"commissionerAndGoal": {"referenceToCommissioner": [{"shortDescription": [{"value": "Amorim Revestimentos, S. A.", "lang": "en"}], "type": "contact data set", "refObjectId": "0871e612-de2a-429d-bced-1f175ad31e0d", "uri": "../contacts/0871e612-de2a-429d-bced-1f175ad31e0d.xml"}]}, "dataGenerator": {"referenceToPersonOrEntityGeneratingTheDataSet": [{"shortDescription": [{"value": "Amorim Revestimentos, S. A.", "lang": "en"}], "type": "contact data set", "refObjectId": "0871e612-de2a-429d-bced-1f175ad31e0d", "uri": "../contacts/0871e612-de2a-429d-bced-1f175ad31e0d.xml"}]}, "dataEntryBy": {"timeStamp": 1670403679658, "referenceToDataSetFormat": [{"shortDescription": [{"value": "ILCD Format", "lang": "en"}], "type": "source data set", "refObjectId": "a97a0155-0234-4b87-b4ce-a45da52f2a40", "uri": "../sources/a97a0155-0234-4b87-b4ce-a45da52f2a40.xml"}, {"shortDescription": [{"value": "EPD-Datenformaterweiterungen v1.2", "lang": "de"}, {"value": "EPD Data Format Extensions v1.2", "lang": "en"}], "type": "source data set", "refObjectId": "a29449fd-aa2f-4de8-b5d7-4b06b43c6fde", "uri": "../sources/a29449fd-aa2f-4de8-b5d7-4b06b43c6fde.xml"}]}, "publicationAndOwnership": {"dataSetVersion": "00.02.000", "referenceToRegistrationAuthority": {"shortDescription": [{"value": "Institut Bauen und Umwelt e. V.", "lang": "en"}], "type": "contact data set", "refObjectId": "d111dbec-b024-4be5-86c5-752d6eb2cf95", "uri": "../contacts/d111dbec-b024-4be5-86c5-752d6eb2cf95.xml"}, "registrationNumber": "EPD-ACF-20220041-ICA1-EN", "referenceToOwnershipOfDataSet": {"shortDescription": [{"value": "Amorim Revestimentos, S. A.", "lang": "en"}], "type": "contact data set", "refObjectId": "0871e612-de2a-429d-bced-1f175ad31e0d", "uri": "../contacts/0871e612-de2a-429d-bced-1f175ad31e0d.xml"}, "copyright": true, "licenseType": "Free of charge for all users and uses", "accessRestrictions": [{"value": "None", "lang": "en"}], "other": {"anies": [{"name": "referenceToPublisher", "value": {"shortDescription": [{"value": "Institut Bauen und Umwelt e. V.", "lang": "en"}], "type": "contact data set", "refObjectId": "d111dbec-b024-4be5-86c5-752d6eb2cf95", "uri": "../contacts/d111dbec-b024-4be5-86c5-752d6eb2cf95.xml"}}]}}}, "exchanges": {"exchange": [{"dataSetInternalID": 0, "referenceToFlowDataSet": {"shortDescription": [{"value": "Amorim Wise Cork Pure PU PF (Amorim Wise Cork Pure PU PF)", "lang": "en"}], "type": "flow data set", "refObjectId": "4018493b-0b0b-0051-4e21-887f2af25c3e", "uri": "../flows/4018493b-0b0b-0051-4e21-887f2af25c3e.xml"}, "meanAmount": 1.0, "referencesToDataSource": {}, "referenceFlow": true, "resolvedFlowVersion": "00.02.000", "resultingflowAmount": 1.0, "flowProperties": [{"name": [{"lang": "en", "value": "Area"}, {"lang": "de", "value": "Fläche"}], "uuid": "93a60a56-a3c8-19da-a746-0800200c9a66", "referenceFlowProperty": true, "meanValue": 1.0, "referenceUnit": "qm", "unitGroupUUID": "c20a03d7-bd90-4569-bc94-66cfd364dfc8"}], "materialProperties": [{"name": "layer thickness", "value": "0.004", "unit": "m", "unitDescription": "meters"}, {"name": "grammage", "value": "2.1", "unit": "kg/m^2", "unitDescription": "kilograms per square meter"}, {"name": "conversion factor [mass/declared unit]", "value": "0.48", "unit": "-", "unitDescription": "Without unit"}, {"name": "gross density", "value": "525.0", "unit": "kg/m^3", "unitDescription": "kilograms per cubic metre"}], "typeOfFlow": "Product flow", "classification": {"classHierarchy": "Holz / Holzböden / Mehrschichtig modulare Bodenbeläge", "name": "OEKOBAU.DAT"}}, {"dataSetInternalID": 1, "referenceToFlowDataSet": {"shortDescription": [{"value": "Renewable primary energy as energy carrier (PERE)", "lang": "en"}, {"value": "Erneuerbare Primärenergie als Energieträger (PERE)", "lang": "de"}], "type": "flow data set", "refObjectId": "20f32be5-0398-4288-9b6d-accddd195317", "uri": "../flows/20f32be5-0398-4288-9b6d-accddd195317.xml"}, "exchange direction": "INPUT", "other": {"anies": [{"name": "referenceToUnitGroupDataSet", "value": {"shortDescription": [{"value": "MJ", "lang": "en"}], "type": "unit group data set", "refObjectId": "93a60a57-a3c8-11da-a746-0800200c9a66", "uri": "../unitgroups/93a60a57-a3c8-11da-a746-0800200c9a66.xml"}}, {"value": "1.6", "module": "A1-A3"}, {"value": "0.0369", "module": "A4"}, {"value": "0.0469", "module": "A5"}, {"value": "0.149", "module": "B2"}, {"value": "0", "module": "C1"}, {"value": "0.00291", "module": "C2", "scenario": "S0"}, {"value": "0.00291", "module": "C2", "scenario": "S1"}, {"value": "0.00291", "module": "C2", "scenario": "S2"}, {"value": "17.2", "module": "C3", "scenario": "S0"}, {"value": "43", "module": "C3", "scenario": "S1"}, {"value": "0.00696", "module": "C4", "scenario": "S0"}, {"value": "0.0116", "module": "C4", "scenario": "S2"}, {"value": "-12.3", "module": "D", "scenario": "S0"}, {"value": "-8.61", "module": "D", "scenario": "S1"}, {"value": "-14.8", "module": "D", "scenario": "S2"}]}, "resolvedFlowVersion": "38.00.000", "flowProperties": [], "typeOfFlow": "Other flow", "classification": {"classHierarchy": "Quantities", "name": "GaBiCategories"}}, {"dataSetInternalID": 2, "referenceToFlowDataSet": {"shortDescription": [{"value": "Renewable primary energy resources as material utilization (PERM)", "lang": "en"}, {"value": "Erneuerbare Primärenergie zur stofflichen Nutzung (PERM)", "lang": "de"}], "type": "flow data set", "refObjectId": "fb3ec0de-548d-4508-aea5-00b73bf6f702", "uri": "../flows/fb3ec0de-548d-4508-aea5-00b73bf6f702.xml"}, "exchange direction": "INPUT", "other": {"anies": [{"name": "referenceToUnitGroupDataSet", "value": {"shortDescription": [{"value": "MJ", "lang": "en"}], "type": "unit group data set", "refObjectId": "93a60a57-a3c8-11da-a746-0800200c9a66", "uri": "../unitgroups/93a60a57-a3c8-11da-a746-0800200c9a66.xml"}}, {"value": "43", "module": "A1-A3"}, {"value": "0", "module": "A4"}, {"value": "-0.363", "module": "A5"}, {"value": "0.0716", "module": "B2"}, {"value": "0", "module": "C1"}, {"value": "0", "module": "C2", "scenario": "S0"}, {"value": "0", "module": "C2", "scenario": "S1"}, {"value": "0", "module": "C2", "scenario": "S2"}, {"value": "-17", "module": "C3", "scenario": "S0"}, {"value": "-42.6", "module": "C3", "scenario": "S1"}, {"value": "0", "module": "C4", "scenario": "S0"}, {"value": "0", "module": "C4", "scenario": "S2"}, {"value": "-5.93", "module": "D", "scenario": "S0"}, {"value": "-14.8", "module": "D", "scenario": "S1"}, {"value": "0", "module": "D", "scenario": "S2"}]}, "resolvedFlowVersion": "38.00.000", "flowProperties": [], "typeOfFlow": "Other flow", "classification": {"classHierarchy": "Quantities", "name": "GaBiCategories"}}, {"dataSetInternalID": 3, "referenceToFlowDataSet": {"shortDescription": [{"value": "Total use of renewable primary energy resources (PERT)", "lang": "en"}, {"value": "Total erneuerbare Primärenergie (PERT)", "lang": "de"}], "type": "flow data set", "refObjectId": "53f97275-fa8a-4cdd-9024-65936002acd0", "uri": "../flows/53f97275-fa8a-4cdd-9024-65936002acd0.xml"}, "exchange direction": "INPUT", "other": {"anies": [{"name": "referenceToUnitGroupDataSet", "value": {"shortDescription": [{"value": "MJ", "lang": "en"}], "type": "unit group data set", "refObjectId": "93a60a57-a3c8-11da-a746-0800200c9a66", "uri": "../unitgroups/93a60a57-a3c8-11da-a746-0800200c9a66.xml"}}, {"value": "44.6", "module": "A1-A3"}, {"value": "0.0369", "module": "A4"}, {"value": "-0.316", "module": "A5"}, {"value": "2.21", "module": "B2"}, {"value": "0", "module": "C1"}, {"value": "0.00291", "module": "C2", "scenario": "S0"}, {"value": "0.00291", "module": "C2", "scenario": "S1"}, {"value": "0.00291", "module": "C2", "scenario": "S2"}, {"value": "0.2", "module": "C3", "scenario": "S0"}, {"value": "0.4", "module": "C3", "scenario": "S1"}, {"value": "0.00696", "module": "C4", "scenario": "S0"}, {"value": "0.0116", "module": "C4", "scenario": "S2"}, {"value": "-18.3", "module": "D", "scenario": "S0"}, {"value": "-23.4", "module": "D", "scenario": "S1"}, {"value": "-14.8", "module": "D", "scenario": "S2"}]}, "resolvedFlowVersion": "38.00.000", "flowProperties": [], "typeOfFlow": "Other flow", "classification": {"classHierarchy": "Quantities / Environmental quantities / EPD EN 15804 / LCI indicators", "name": "GaBiCategories"}}, {"dataSetInternalID": 4, "referenceToFlowDataSet": {"shortDescription": [{"value": "Non renewable primary energy as energy carrier (PENRE)", "lang": "en"}, {"value": "Nicht-erneuerbare Primärenergie als Energieträger (PENRE)", "lang": "de"}], "type": "flow data set", "refObjectId": "ac857178-2b45-46ec-892a-a9a4332f0372", "uri": "../flows/ac857178-2b45-46ec-892a-a9a4332f0372.xml"}, "exchange direction": "INPUT", "other": {"anies": [{"name": "referenceToUnitGroupDataSet", "value": {"shortDescription": [{"value": "MJ", "lang": "en"}], "type": "unit group data set", "refObjectId": "93a60a57-a3c8-11da-a746-0800200c9a66", "uri": "../unitgroups/93a60a57-a3c8-11da-a746-0800200c9a66.xml"}}, {"value": "4.76", "module": "A1-A3"}, {"value": "2.39", "module": "A4"}, {"value": "0.204", "module": "A5"}, {"value": "0.925", "module": "B2"}, {"value": "0", "module": "C1"}, {"value": "0.266", "module": "C2", "scenario": "S0"}, {"value": "0.266", "module": "C2", "scenario": "S1"}, {"value": "0.266", "module": "C2", "scenario": "S2"}, {"value": "7.42", "module": "C3", "scenario": "S0"}, {"value": "18.5", "module": "C3", "scenario": "S1"}, {"value": "0.417", "module": "C4", "scenario": "S0"}, {"value": "0.695", "module": "C4", "scenario": "S2"}, {"value": "-26.1", "module": "D", "scenario": "S0"}, {"value": "-53.4", "module": "D", "scenario": "S1"}, {"value": "-7.93", "module": "D", "scenario": "S2"}]}, "resolvedFlowVersion": "38.00.000", "flowProperties": [], "typeOfFlow": "Other flow", "classification": {"classHierarchy": "Quantities", "name": "GaBiCategories"}}, {"dataSetInternalID": 5, "referenceToFlowDataSet": {"shortDescription": [{"value": "Non renewable primary energy as material utilization (PENRM)", "lang": "en"}, {"value": "Nicht-erneuerbare Primärenergie zur stofflichen Nutzung (PENRM)", "lang": "de"}], "type": "flow data set", "refObjectId": "1421caa0-679d-4bf4-b282-0eb850ccae27", "uri": "../flows/1421caa0-679d-4bf4-b282-0eb850ccae27.xml"}, "exchange direction": "INPUT", "other": {"anies": [{"name": "referenceToUnitGroupDataSet", "value": {"shortDescription": [{"value": "MJ", "lang": "en"}], "type": "unit group data set", "refObjectId": "93a60a57-a3c8-11da-a746-0800200c9a66", "uri": "../unitgroups/93a60a57-a3c8-11da-a746-0800200c9a66.xml"}}, {"value": "18.2", "module": "A1-A3"}, {"value": "0", "module": "A4"}, {"value": "-4.48", "module": "A5"}, {"value": "1.45", "module": "B2"}, {"value": "0", "module": "C1"}, {"value": "0", "module": "C2", "scenario": "S0"}, {"value": "0", "module": "C2", "scenario": "S1"}, {"value": "0", "module": "C2", "scenario": "S2"}, {"value": "-5.48", "module": "C3", "scenario": "S0"}, {"value": "-13.7", "module": "C3", "scenario": "S1"}, {"value": "0", "module": "C4", "scenario": "S0"}, {"value": "0", "module": "C4", "scenario": "S2"}, {"value": "-3.17", "module": "D", "scenario": "S0"}, {"value": "-7.93", "module": "D", "scenario": "S1"}, {"value": "0", "module": "D", "scenario": "S2"}]}, "resolvedFlowVersion": "38.00.000", "flowProperties": [], "typeOfFlow": "Other flow", "classification": {"classHierarchy": "Quantities", "name": "GaBiCategories"}}, {"dataSetInternalID": 6, "referenceToFlowDataSet": {"shortDescription": [{"value": "Total use of non renewable primary energy resources (PENRT)", "lang": "en"}, {"value": "Total nicht erneuerbare Primärenergie (PENRT)", "lang": "de"}], "type": "flow data set", "refObjectId": "06159210-646b-4c8d-8583-da9b3b95a6c1", "uri": "../flows/06159210-646b-4c8d-8583-da9b3b95a6c1.xml"}, "exchange direction": "INPUT", "other": {"anies": [{"name": "referenceToUnitGroupDataSet", "value": {"shortDescription": [{"value": "MJ", "lang": "en"}], "type": "unit group data set", "refObjectId": "93a60a57-a3c8-11da-a746-0800200c9a66", "uri": "../unitgroups/93a60a57-a3c8-11da-a746-0800200c9a66.xml"}}, {"value": "23", "module": "A1-A3"}, {"value": "2.39", "module": "A4"}, {"value": "-4.28", "module": "A5"}, {"value": "2.37", "module": "B2"}, {"value": "0", "module": "C1"}, {"value": "0.266", "module": "C2", "scenario": "S0"}, {"value": "0.266", "module": "C2", "scenario": "S1"}, {"value": "0.266", "module": "C2", "scenario": "S2"}, {"value": "1.94", "module": "C3", "scenario": "S0"}, {"value": "4.8", "module": "C3", "scenario": "S1"}, {"value": "0.417", "module": "C4", "scenario": "S0"}, {"value": "0.695", "module": "C4", "scenario": "S2"}, {"value": "-29.3", "module": "D", "scenario": "S0"}, {"value": "-61.3", "module": "D", "scenario": "S1"}, {"value": "-7.93", "module": "D", "scenario": "S2"}]}, "resolvedFlowVersion": "38.00.000", "flowProperties": [], "typeOfFlow": "Other flow", "classification": {"classHierarchy": "Quantities / Environmental quantities / EPD EN 15804 / LCI indicators", "name": "GaBiCategories"}}, {"dataSetInternalID": 7, "referenceToFlowDataSet": {"shortDescription": [{"value": "Use of secondary material (SM)", "lang": "en"}, {"value": "Einsatz von Sekundärstoffen (SM)", "lang": "de"}], "type": "flow data set", "refObjectId": "c6a1f35f-2d09-4f54-8dfb-97e502e1ce92", "uri": "../flows/c6a1f35f-2d09-4f54-8dfb-97e502e1ce92.xml"}, "exchange direction": "INPUT", "other": {"anies": [{"name": "referenceToUnitGroupDataSet", "value": {"shortDescription": [{"value": "kg", "lang": "en"}], "type": "unit group data set", "refObjectId": "ad38d542-3fe9-439d-9b95-2f5f7752acaf", "uri": "../unitgroups/ad38d542-3fe9-439d-9b95-2f5f7752acaf.xml"}}, {"value": "0", "module": "A1-A3"}, {"value": "0", "module": "A4"}, {"value": "0", "module": "A5"}, {"value": "0", "module": "B2"}, {"value": "0", "module": "C1"}, {"value": "0", "module": "C2", "scenario": "S0"}, {"value": "0", "module": "C2", "scenario": "S1"}, {"value": "0", "module": "C2", "scenario": "S2"}, {"value": "0", "module": "C3", "scenario": "S0"}, {"value": "0", "module": "C3", "scenario": "S1"}, {"value": "0", "module": "C4", "scenario": "S0"}, {"value": "0", "module": "C4", "scenario": "S2"}, {"value": "0.457", "module": "D", "scenario": "S0"}, {"value": "0.457", "module": "D", "scenario": "S1"}, {"value": "0.457", "module": "D", "scenario": "S2"}]}, "resolvedFlowVersion": "38.00.000", "flowProperties": [], "typeOfFlow": "Other flow", "classification": {"classHierarchy": "Quantities / Environmental quantities / EPD EN 15804 / LCI indicators", "name": "GaBiCategories"}}, {"dataSetInternalID": 8, "referenceToFlowDataSet": {"shortDescription": [{"value": "Use of renewable secondary fuels (RSF)", "lang": "en"}, {"value": "Erneuerbare Sekundärbrennstoffe (RSF)", "lang": "de"}], "type": "flow data set", "refObjectId": "64333088-a55f-4aa2-9a31-c10b07816787", "uri": "../flows/64333088-a55f-4aa2-9a31-c10b07816787.xml"}, "exchange direction": "INPUT", "other": {"anies": [{"name": "referenceToUnitGroupDataSet", "value": {"shortDescription": [{"value": "MJ", "lang": "en"}], "type": "unit group data set", "refObjectId": "93a60a57-a3c8-11da-a746-0800200c9a66", "uri": "../unitgroups/93a60a57-a3c8-11da-a746-0800200c9a66.xml"}}, {"value": "0", "module": "A1-A3"}, {"value": "0", "module": "A4"}, {"value": "0", "module": "A5"}, {"value": "0", "module": "B2"}, {"value": "0", "module": "C1"}, {"value": "0", "module": "C2", "scenario": "S0"}, {"value": "0", "module": "C2", "scenario": "S1"}, {"value": "0", "module": "C2", "scenario": "S2"}, {"value": "0", "module": "C3", "scenario": "S0"}, {"value": "0", "module": "C3", "scenario": "S1"}, {"value": "0", "module": "C4", "scenario": "S0"}, {"value": "0", "module": "C4", "scenario": "S2"}, {"value": "0", "module": "D", "scenario": "S0"}, {"value": "0", "module": "D", "scenario": "S1"}, {"value": "0", "module": "D", "scenario": "S2"}]}, "resolvedFlowVersion": "38.00.000", "flowProperties": [], "typeOfFlow": "Other flow", "classification": {"classHierarchy": "Quantities / Environmental quantities / EPD EN 15804 / LCI indicators", "name": "GaBiCategories"}}, {"dataSetInternalID": 9, "referenceToFlowDataSet": {"shortDescription": [{"value": "Use of non renewable secondary fuels (NRSF)", "lang": "en"}, {"value": "Nicht erneuerbare Sekundärbrennstoffe (NRSF)", "lang": "de"}], "type": "flow data set", "refObjectId": "89def144-d39a-4287-b86f-efde453ddcb2", "uri": "../flows/89def144-d39a-4287-b86f-efde453ddcb2.xml"}, "exchange direction": "INPUT", "other": {"anies": [{"name": "referenceToUnitGroupDataSet", "value": {"shortDescription": [{"value": "MJ", "lang": "en"}], "type": "unit group data set", "refObjectId": "93a60a57-a3c8-11da-a746-0800200c9a66", "uri": "../unitgroups/93a60a57-a3c8-11da-a746-0800200c9a66.xml"}}, {"value": "0", "module": "A1-A3"}, {"value": "0", "module": "A4"}, {"value": "0", "module": "A5"}, {"value": "0", "module": "B2"}, {"value": "0", "module": "C1"}, {"value": "0", "module": "C2", "scenario": "S0"}, {"value": "0", "module": "C2", "scenario": "S1"}, {"value": "0", "module": "C2", "scenario": "S2"}, {"value": "0", "module": "C3", "scenario": "S0"}, {"value": "0", "module": "C3", "scenario": "S1"}, {"value": "0", "module": "C4", "scenario": "S0"}, {"value": "0", "module": "C4", "scenario": "S2"}, {"value": "0", "module": "D", "scenario": "S0"}, {"value": "0", "module": "D", "scenario": "S1"}, {"value": "0", "module": "D", "scenario": "S2"}]}, "resolvedFlowVersion": "38.00.000", "flowProperties": [], "typeOfFlow": "Other flow", "classification": {"classHierarchy": "Quantities / Environmental quantities / EPD EN 15804 / LCI indicators", "name": "GaBiCategories"}}, {"dataSetInternalID": 10, "referenceToFlowDataSet": {"shortDescription": [{"value": "Use of net fresh water (FW)", "lang": "en"}, {"value": "Einsatz von Süßwasserressourcen (FW)", "lang": "de"}], "type": "flow data set", "refObjectId": "3cf952c8-f3a4-461d-8c96-96456ca62246", "uri": "../flows/3cf952c8-f3a4-461d-8c96-96456ca62246.xml"}, "exchange direction": "INPUT", "other": {"anies": [{"name": "referenceToUnitGroupDataSet", "value": {"shortDescription": [{"value": "m^3", "lang": "en"}], "type": "unit group data set", "refObjectId": "cd950537-0a98-4044-9ba7-9f9a68d0a504", "uri": "../unitgroups/cd950537-0a98-4044-9ba7-9f9a68d0a504.xml"}}, {"value": "0.133949272053826", "module": "A1-A3"}, {"value": "0.00233336572516898", "module": "A4"}, {"value": "0.0282364015978551", "module": "A5"}, {"value": "0.0119412863124908", "module": "B2"}, {"value": "0.000197780470668481", "module": "C1"}, {"value": "0.000197780470668481", "module": "C2", "scenario": "S0"}, {"value": "0.000197780470668481", "module": "C2", "scenario": "S1"}, {"value": "0.000197780470668481", "module": "C2", "scenario": "S2"}, {"value": "0.000642904815934006", "module": "C3", "scenario": "S0"}, {"value": "0.00160726203983502", "module": "C3", "scenario": "S1"}, {"value": "0.000772087986642454", "module": "C4", "scenario": "S0"}, {"value": "0.00128681331107076", "module": "C4", "scenario": "S2"}, {"value": "-0.23349933375942", "module": "D", "scenario": "S0"}, {"value": "-0.489011514325064", "module": "D", "scenario": "S1"}, {"value": "-0.0631578800489909", "module": "D", "scenario": "S2"}]}, "resolvedFlowVersion": "38.00.000", "flowProperties": [], "typeOfFlow": "Other flow", "classification": {"classHierarchy": "Quantities / Environmental quantities / EPD EN 15804 / LCI indicators", "name": "GaBiCategories"}}, {"dataSetInternalID": 11, "referenceToFlowDataSet": {"shortDescription": [{"value": "Hazardous waste disposed (HWD)", "lang": "en"}, {"value": "Gefährlicher Abfall zur Deponie (HWD)", "lang": "de"}], "type": "flow data set", "refObjectId": "430f9e0f-59b2-46a0-8e0d-55e0e84948fc", "uri": "../flows/430f9e0f-59b2-46a0-8e0d-55e0e84948fc.xml"}, "exchange direction": "OUTPUT", "other": {"anies": [{"name": "referenceToUnitGroupDataSet", "value": {"shortDescription": [{"value": "kg", "lang": "en"}], "type": "unit group data set", "refObjectId": "ad38d542-3fe9-439d-9b95-2f5f7752acaf", "uri": "../unitgroups/ad38d542-3fe9-439d-9b95-2f5f7752acaf.xml"}}, {"value": "1.92147052707056E-05", "module": "A1-A3"}, {"value": "1.41773244264947E-06", "module": "A4"}, {"value": "4.26197794751045E-06", "module": "A5"}, {"value": "8.61107457894585E-08", "module": "B2"}, {"value": "0", "module": "C1"}, {"value": "1.54836981902662E-07", "module": "C2", "scenario": "S0"}, {"value": "1.54836981902662E-07", "module": "C2", "scenario": "S1"}, {"value": "1.54836981902662E-07", "module": "C2", "scenario": "S2"}, {"value": "2.98899310919864E-07", "module": "C3", "scenario": "S0"}, {"value": "7.47248277299661E-07", "module": "C3", "scenario": "S1"}, {"value": "3.24849195856292E-07", "module": "C4", "scenario": "S0"}, {"value": "5.41415326427153E-07", "module": "C4", "scenario": "S2"}, {"value": "-3.44508548103626E-05", "module": "D", "scenario": "S0"}, {"value": "-7.0817992558748E-05", "module": "D", "scenario": "S1"}, {"value": "-1.0206096311439E-05", "module": "D", "scenario": "S2"}]}, "resolvedFlowVersion": "38.00.000", "flowProperties": [], "typeOfFlow": "Other flow", "classification": {"classHierarchy": "Quantities / Environmental quantities / EPD EN 15804 / LCI indicators", "name": "GaBiCategories"}}, {"dataSetInternalID": 12, "referenceToFlowDataSet": {"shortDescription": [{"value": "Non hazardous waste disposed (NHWD)", "lang": "en"}, {"value": "Entsorgter nicht gefährlicher Abfall (NHWD)", "lang": "de"}], "type": "flow data set", "refObjectId": "b29ef66b-e286-4afa-949f-62f1a7b4d7fa", "uri": "../flows/b29ef66b-e286-4afa-949f-62f1a7b4d7fa.xml"}, "exchange direction": "OUTPUT", "other": {"anies": [{"name": "referenceToUnitGroupDataSet", "value": {"shortDescription": [{"value": "kg", "lang": "en"}], "type": "unit group data set", "refObjectId": "ad38d542-3fe9-439d-9b95-2f5f7752acaf", "uri": "../unitgroups/ad38d542-3fe9-439d-9b95-2f5f7752acaf.xml"}}, {"value": "0.275287059238981", "module": "A1-A3"}, {"value": "0.0746397773295177", "module": "A4"}, {"value": "0.648610487882952", "module": "A5"}, {"value": "0.000445190303577281", "module": "B2"}, {"value": "0", "module": "C1"}, {"value": "0.0125501770746638", "module": "C2", "scenario": "S0"}, {"value": "0.0125501770746638", "module": "C2", "scenario": "S1"}, {"value": "0.0125501770746638", "module": "C2", "scenario": "S2"}, {"value": "0.0179996697032238", "module": "C3", "scenario": "S0"}, {"value": "0.0449991742580594", "module": "C3", "scenario": "S1"}, {"value": "1.53740457987455", "module": "C4", "scenario": "S0"}, {"value": "2.56234096645759", "module": "C4", "scenario": "S2"}, {"value": "-0.152905699627997", "module": "D", "scenario": "S0"}, {"value": "-0.271085405642915", "module": "D", "scenario": "S1"}, {"value": "-0.0741192289513846", "module": "D", "scenario": "S2"}]}, "resolvedFlowVersion": "38.00.000", "flowProperties": [], "typeOfFlow": "Other flow", "classification": {"classHierarchy": "Quantities / Environmental quantities / EPD EN 15804 / LCI indicators", "name": "GaBiCategories"}}, {"dataSetInternalID": 13, "referenceToFlowDataSet": {"shortDescription": [{"value": "Radioactive waste disposed (RWD)", "lang": "en"}, {"value": "Entsorgter radioaktiver Abfall (RWD)", "lang": "de"}], "type": "flow data set", "refObjectId": "3449546e-52ad-4b39-b809-9fb77cea8ff6", "uri": "../flows/3449546e-52ad-4b39-b809-9fb77cea8ff6.xml"}, "exchange direction": "OUTPUT", "other": {"anies": [{"name": "referenceToUnitGroupDataSet", "value": {"shortDescription": [{"value": "kg", "lang": "en"}], "type": "unit group data set", "refObjectId": "ad38d542-3fe9-439d-9b95-2f5f7752acaf", "uri": "../unitgroups/ad38d542-3fe9-439d-9b95-2f5f7752acaf.xml"}}, {"value": "6.78032930498879E-05", "module": "A1-A3"}, {"value": "1.59597960649995E-05", "module": "A4"}, {"value": "1.6075442618777E-05", "module": "A5"}, {"value": "4.04598647921698E-07", "module": "B2"}, {"value": "0", "module": "C1"}, {"value": "1.7992779992957E-06", "module": "C2", "scenario": "S0"}, {"value": "1.7992779992957E-06", "module": "C2", "scenario": "S1"}, {"value": "1.7992779992957E-06", "module": "C2", "scenario": "S2"}, {"value": "3.22443423532238E-07", "module": "C3", "scenario": "S0"}, {"value": "8.06108558830594E-07", "module": "C3", "scenario": "S1"}, {"value": "2.52092265976002E-06", "module": "C4", "scenario": "S0"}, {"value": "4.2015377662667E-06", "module": "C4", "scenario": "S2"}, {"value": "-0.00018336833238807", "module": "D", "scenario": "S0"}, {"value": "-0.000418764618071016", "module": "D", "scenario": "S1"}, {"value": "-2.64374752661066E-05", "module": "D", "scenario": "S2"}]}, "resolvedFlowVersion": "38.00.000", "flowProperties": [], "typeOfFlow": "Other flow", "classification": {"classHierarchy": "Quantities / Environmental quantities / EPD EN 15804 / LCI indicators", "name": "GaBiCategories"}}, {"dataSetInternalID": 14, "referenceToFlowDataSet": {"shortDescription": [{"value": "Components for re-use (CRU)", "lang": "en"}, {"value": "Komponenten für die Wiederverwendung (CRU)", "lang": "de"}], "type": "flow data set", "refObjectId": "a2b32f97-3fc7-4af2-b209-525bc6426f33", "uri": "../flows/a2b32f97-3fc7-4af2-b209-525bc6426f33.xml"}, "exchange direction": "OUTPUT", "other": {"anies": [{"name": "referenceToUnitGroupDataSet", "value": {"shortDescription": [{"value": "kg", "lang": "en"}], "type": "unit group data set", "refObjectId": "ad38d542-3fe9-439d-9b95-2f5f7752acaf", "uri": "../unitgroups/ad38d542-3fe9-439d-9b95-2f5f7752acaf.xml"}}, {"value": "0.322627264850925", "module": "A1-A3"}, {"value": "0", "module": "A4"}, {"value": "0", "module": "A5"}, {"value": "0", "module": "B2"}, {"value": "0", "module": "C1"}, {"value": "0", "module": "C2", "scenario": "S0"}, {"value": "0", "module": "C2", "scenario": "S1"}, {"value": "0", "module": "C2", "scenario": "S2"}, {"value": "0", "module": "C3", "scenario": "S0"}, {"value": "0", "module": "C3", "scenario": "S1"}, {"value": "0", "module": "C4", "scenario": "S0"}, {"value": "0", "module": "C4", "scenario": "S2"}, {"value": "0", "module": "D", "scenario": "S0"}, {"value": "0", "module": "D", "scenario": "S1"}, {"value": "0", "module": "D", "scenario": "S2"}]}, "resolvedFlowVersion": "38.00.000", "flowProperties": [], "typeOfFlow": "Other flow", "classification": {"classHierarchy": "Quantities / Environmental quantities / EPD EN 15804 / LCI indicators", "name": "GaBiCategories"}}, {"dataSetInternalID": 15, "referenceToFlowDataSet": {"shortDescription": [{"value": "Materials for recycling (MFR)", "lang": "en"}, {"value": "Stoffe zum Recycling (MFR)", "lang": "de"}], "type": "flow data set", "refObjectId": "d7fe48a5-4103-49c8-9aae-b0b5dfdbd6ae", "uri": "../flows/d7fe48a5-4103-49c8-9aae-b0b5dfdbd6ae.xml"}, "exchange direction": "OUTPUT", "other": {"anies": [{"name": "referenceToUnitGroupDataSet", "value": {"shortDescription": [{"value": "kg", "lang": "en"}], "type": "unit group data set", "refObjectId": "ad38d542-3fe9-439d-9b95-2f5f7752acaf", "uri": "../unitgroups/ad38d542-3fe9-439d-9b95-2f5f7752acaf.xml"}}, {"value": "0.127574876528032", "module": "A1-A3"}, {"value": "0", "module": "A4"}, {"value": "0.4611", "module": "A5"}, {"value": "0", "module": "B2"}, {"value": "0", "module": "C1"}, {"value": "0", "module": "C2", "scenario": "S0"}, {"value": "0", "module": "C2", "scenario": "S1"}, {"value": "0", "module": "C2", "scenario": "S2"}, {"value": "0", "module": "C3", "scenario": "S0"}, {"value": "0", "module": "C3", "scenario": "S1"}, {"value": "0", "module": "C4", "scenario": "S0"}, {"value": "0", "module": "C4", "scenario": "S2"}, {"value": "0", "module": "D", "scenario": "S0"}, {"value": "0", "module": "D", "scenario": "S1"}, {"value": "0", "module": "D", "scenario": "S2"}]}, "resolvedFlowVersion": "38.00.000", "flowProperties": [], "typeOfFlow": "Other flow", "classification": {"classHierarchy": "Quantities / Environmental quantities / EPD EN 15804 / LCI indicators", "name": "GaBiCategories"}}, {"dataSetInternalID": 16, "referenceToFlowDataSet": {"shortDescription": [{"value": "Materials for energy recovery (MER)", "lang": "en"}, {"value": "Stoffe für die Energierückgewinnung (MER)", "lang": "de"}], "type": "flow data set", "refObjectId": "59a9181c-3aaf-46ee-8b13-2b3723b6e447", "uri": "../flows/59a9181c-3aaf-46ee-8b13-2b3723b6e447.xml"}, "exchange direction": "OUTPUT", "other": {"anies": [{"name": "referenceToUnitGroupDataSet", "value": {"shortDescription": [{"value": "kg", "lang": "en"}], "type": "unit group data set", "refObjectId": "ad38d542-3fe9-439d-9b95-2f5f7752acaf", "uri": "../unitgroups/ad38d542-3fe9-439d-9b95-2f5f7752acaf.xml"}}, {"value": "4.43560986786929", "module": "A1-A3"}, {"value": "0", "module": "A4"}, {"value": "0", "module": "A5"}, {"value": "0", "module": "B2"}, {"value": "0", "module": "C1"}, {"value": "0", "module": "C2", "scenario": "S0"}, {"value": "0", "module": "C2", "scenario": "S1"}, {"value": "0", "module": "C2", "scenario": "S2"}, {"value": "0", "module": "C3", "scenario": "S0"}, {"value": "0", "module": "C3", "scenario": "S1"}, {"value": "0", "module": "C4", "scenario": "S0"}, {"value": "0", "module": "C4", "scenario": "S2"}, {"value": "0.84", "module": "D", "scenario": "S0"}, {"value": "2.1", "module": "D", "scenario": "S1"}, {"value": "0", "module": "D", "scenario": "S2"}]}, "resolvedFlowVersion": "38.00.000", "flowProperties": [], "typeOfFlow": "Other flow", "classification": {"classHierarchy": "Quantities / Environmental quantities / EPD EN 15804 / LCI indicators", "name": "GaBiCategories"}}, {"dataSetInternalID": 17, "referenceToFlowDataSet": {"shortDescription": [{"value": "Exported electrical energy (EEE)", "lang": "en"}, {"value": "Exportierte elektrische Energie (EEE)", "lang": "de"}], "type": "flow data set", "refObjectId": "4da0c987-2b76-40d6-9e9e-82a017aaaf29", "uri": "../flows/4da0c987-2b76-40d6-9e9e-82a017aaaf29.xml"}, "exchange direction": "OUTPUT", "other": {"anies": [{"name": "referenceToUnitGroupDataSet", "value": {"shortDescription": [{"value": "MJ", "lang": "en"}], "type": "unit group data set", "refObjectId": "93a60a57-a3c8-11da-a746-0800200c9a66", "uri": "../unitgroups/93a60a57-a3c8-11da-a746-0800200c9a66.xml"}}, {"value": "0", "module": "A1-A3"}, {"value": "0", "module": "A4"}, {"value": "0", "module": "A5"}, {"value": "0", "module": "B2"}, {"value": "0", "module": "C1"}, {"value": "0", "module": "C2", "scenario": "S0"}, {"value": "0", "module": "C2", "scenario": "S1"}, {"value": "0", "module": "C2", "scenario": "S2"}, {"value": "8.44032", "module": "C3", "scenario": "S0"}, {"value": "21.1008", "module": "C3", "scenario": "S1"}, {"value": "0", "module": "C4", "scenario": "S0"}, {"value": "0", "module": "C4", "scenario": "S2"}, {"value": "0", "module": "D", "scenario": "S0"}, {"value": "0", "module": "D", "scenario": "S1"}, {"value": "0", "module": "D", "scenario": "S2"}]}, "resolvedFlowVersion": "38.00.000", "flowProperties": [], "typeOfFlow": "Other flow", "classification": {"classHierarchy": "Quantities / Environmental quantities / EPD EN 15804 / LCI indicators", "name": "GaBiCategories"}}, {"dataSetInternalID": 18, "referenceToFlowDataSet": {"shortDescription": [{"value": "Exported thermal energy (EET)", "lang": "en"}, {"value": "Exportierte thermische Energie (EET)", "lang": "de"}], "type": "flow data set", "refObjectId": "98daf38a-7a79-46d3-9a37-2b7bd0955810", "uri": "../flows/98daf38a-7a79-46d3-9a37-2b7bd0955810.xml"}, "exchange direction": "OUTPUT", "other": {"anies": [{"name": "referenceToUnitGroupDataSet", "value": {"shortDescription": [{"value": "MJ", "lang": "en"}], "type": "unit group data set", "refObjectId": "93a60a57-a3c8-11da-a746-0800200c9a66", "uri": "../unitgroups/93a60a57-a3c8-11da-a746-0800200c9a66.xml"}}, {"value": "0", "module": "A1-A3"}, {"value": "0", "module": "A4"}, {"value": "0", "module": "A5"}, {"value": "0", "module": "B2"}, {"value": "0", "module": "C1"}, {"value": "0", "module": "C2", "scenario": "S0"}, {"value": "0", "module": "C2", "scenario": "S1"}, {"value": "0", "module": "C2", "scenario": "S2"}, {"value": "0", "module": "C3", "scenario": "S0"}, {"value": "0", "module": "C3", "scenario": "S1"}, {"value": "0", "module": "C4", "scenario": "S0"}, {"value": "0", "module": "C4", "scenario": "S2"}, {"value": "0", "module": "D", "scenario": "S0"}, {"value": "0", "module": "D", "scenario": "S1"}, {"value": "0", "module": "D", "scenario": "S2"}]}, "resolvedFlowVersion": "38.00.000", "flowProperties": [], "typeOfFlow": "Other flow", "classification": {"classHierarchy": "Quantities / Environmental quantities / EPD EN 15804 / LCI indicators", "name": "GaBiCategories"}}]}, "LCIAResults": {"LCIAResult": [{"referenceToLCIAMethodDataSet": {"shortDescription": [{"value": "Global Warming Potential total (GWP-total)", "lang": "en"}, {"value": "Globales Erwärmungspotenzial total (GWP-total)", "lang": "de"}], "type": "LCIA method data set", "refObjectId": "6a37f984-a4b3-458a-a20a-64418c145fa2", "uri": "../lciamethods/6a37f984-a4b3-458a-a20a-64418c145fa2.xml"}, "other": {"anies": [{"name": "referenceToUnitGroupDataSet", "value": {"shortDescription": [{"value": "kg CO_(2)-Äq.", "lang": "en"}], "type": "unit group data set", "refObjectId": "1ebf3012-d0db-4de2-aefd-ef30cedb0be1", "uri": "../unitgroups/1ebf3012-d0db-4de2-aefd-ef30cedb0be1.xml"}}, {"value": "-2.66", "module": "A1-A3"}, {"value": "0.161", "module": "A4"}, {"value": "0.937", "module": "A5"}, {"value": "0.113", "module": "B2"}, {"value": "0", "module": "C1"}, {"value": "0.0174", "module": "C2", "scenario": "S0"}, {"value": "0.0174", "module": "C2", "scenario": "S1"}, {"value": "0.0174", "module": "C2", "scenario": "S2"}, {"value": "1.36", "module": "C3", "scenario": "S0"}, {"value": "3.41", "module": "C3", "scenario": "S1"}, {"value": "2.17", "module": "C4", "scenario": "S0"}, {"value": "3.61", "module": "C4", "scenario": "S2"}, {"value": "-0.858", "module": "D", "scenario": "S0"}, {"value": "-2.42", "module": "D", "scenario": "S1"}, {"value": "0.184", "module": "D", "scenario": "S2"}]}}, {"referenceToLCIAMethodDataSet": {"shortDescription": [{"value": "Global Warming Potential fossil fuels (GWP-fossil)", "lang": "en"}, {"value": "Globales Erwärmungspotenzial fossil (GWP-fossil)", "lang": "de"}], "type": "LCIA method data set", "refObjectId": "5f635281-343e-44fb-83df-1971b155e6b6", "uri": "../lciamethods/5f635281-343e-44fb-83df-1971b155e6b6.xml"}, "other": {"anies": [{"name": "referenceToUnitGroupDataSet", "value": {"shortDescription": [{"value": "kg CO_(2)-Äq.", "lang": "en"}], "type": "unit group data set", "refObjectId": "1ebf3012-d0db-4de2-aefd-ef30cedb0be1", "uri": "../unitgroups/1ebf3012-d0db-4de2-aefd-ef30cedb0be1.xml"}}, {"value": "1.37", "module": "A1-A3"}, {"value": "0.161", "module": "A4"}, {"value": "0.27", "module": "A5"}, {"value": "0.11", "module": "B2"}, {"value": "0", "module": "C1"}, {"value": "0.0174", "module": "C2", "scenario": "S0"}, {"value": "0.0174", "module": "C2", "scenario": "S1"}, {"value": "0.0174", "module": "C2", "scenario": "S2"}, {"value": "0.0156", "module": "C3", "scenario": "S0"}, {"value": "0.039", "module": "C3", "scenario": "S1"}, {"value": "0.0169", "module": "C4", "scenario": "S0"}, {"value": "0.0282", "module": "C4", "scenario": "S2"}, {"value": "-1.49", "module": "D", "scenario": "S0"}, {"value": "-3.01", "module": "D", "scenario": "S1"}, {"value": "-0.479", "module": "D", "scenario": "S2"}]}}, {"referenceToLCIAMethodDataSet": {"shortDescription": [{"value": "Global Warming Potential biogenic (GWP-biogenic)", "lang": "en"}, {"value": "Globales Erwärmungspotenzial biogen (GWP-biogenic)", "lang": "de"}], "type": "LCIA method data set", "refObjectId": "2356e1ab-0185-4db5-86e5-16de51c7485c", "uri": "../lciamethods/2356e1ab-0185-4db5-86e5-16de51c7485c.xml"}, "other": {"anies": [{"name": "referenceToUnitGroupDataSet", "value": {"shortDescription": [{"value": "kg CO_(2)-Äq.", "lang": "en"}], "type": "unit group data set", "refObjectId": "1ebf3012-d0db-4de2-aefd-ef30cedb0be1", "uri": "../unitgroups/1ebf3012-d0db-4de2-aefd-ef30cedb0be1.xml"}}, {"value": "-4.03", "module": "A1-A3"}, {"value": "7.32E-05", "module": "A4"}, {"value": "0.667", "module": "A5"}, {"value": "-0.00443", "module": "B2"}, {"value": "0", "module": "C1"}, {"value": "4.15E-06", "module": "C2", "scenario": "S0"}, {"value": "4.15E-06", "module": "C2", "scenario": "S1"}, {"value": "4.15E-06", "module": "C2", "scenario": "S2"}, {"value": "1.35", "module": "C3", "scenario": "S0"}, {"value": "3.37", "module": "C3", "scenario": "S1"}, {"value": "2.15", "module": "C4", "scenario": "S0"}, {"value": "3.59", "module": "C4", "scenario": "S2"}, {"value": "0.638", "module": "D", "scenario": "S0"}, {"value": "0.597", "module": "D", "scenario": "S1"}, {"value": "0.666", "module": "D", "scenario": "S2"}]}}, {"referenceToLCIAMethodDataSet": {"shortDescription": [{"value": "Global Warming Potential luluc (GWP-luluc)", "lang": "en"}, {"value": "Globales Erwärmungspotenzial luluc (GWP-luluc)", "lang": "de"}], "type": "LCIA method data set", "refObjectId": "4331bbdb-978a-490d-8707-eeb047f01a55", "uri": "../lciamethods/4331bbdb-978a-490d-8707-eeb047f01a55.xml"}, "other": {"anies": [{"name": "referenceToUnitGroupDataSet", "value": {"shortDescription": [{"value": "kg CO_(2)-Äq.", "lang": "en"}], "type": "unit group data set", "refObjectId": "1ebf3012-d0db-4de2-aefd-ef30cedb0be1", "uri": "../unitgroups/1ebf3012-d0db-4de2-aefd-ef30cedb0be1.xml"}}, {"value": "0.0088", "module": "A1-A3"}, {"value": "6.61E-05", "module": "A4"}, {"value": "0.000378", "module": "A5"}, {"value": "0.008", "module": "B2"}, {"value": "0", "module": "C1"}, {"value": "5.53E-06", "module": "C2", "scenario": "S0"}, {"value": "5.53E-06", "module": "C2", "scenario": "S1"}, {"value": "5.53E-06", "module": "C2", "scenario": "S2"}, {"value": "2.57E-06", "module": "C3", "scenario": "S0"}, {"value": "6.42E-06", "module": "C3", "scenario": "S1"}, {"value": "7.8E-06", "module": "C4", "scenario": "S0"}, {"value": "1.3E-05", "module": "C4", "scenario": "S2"}, {"value": "-0.00545", "module": "D", "scenario": "S0"}, {"value": "-0.00931", "module": "D", "scenario": "S1"}, {"value": "-0.00289", "module": "D", "scenario": "S2"}]}}, {"referenceToLCIAMethodDataSet": {"shortDescription": [{"value": "Depletion potential of the stratospheric ozone layer (ODP)", "lang": "en"}, {"value": "Abbau Potential der stratosphärischen Ozonschicht (ODP)", "lang": "de"}], "type": "LCIA method data set", "refObjectId": "b5c629d6-def3-11e6-bf01-fe55135034f3", "uri": "../lciamethods/b5c629d6-def3-11e6-bf01-fe55135034f3.xml"}, "other": {"anies": [{"name": "referenceToUnitGroupDataSet", "value": {"shortDescription": [{"value": "kg CFC11-Äq.", "lang": "en"}], "type": "unit group data set", "refObjectId": "d9e957c9-7309-4474-bf3a-7777df6c4e5b", "uri": "../unitgroups/d9e957c9-7309-4474-bf3a-7777df6c4e5b.xml"}}, {"value": "1.54919676263774E-07", "module": "A1-A3"}, {"value": "3.48895082882899E-08", "module": "A4"}, {"value": "3.18877767793609E-08", "module": "A5"}, {"value": "6.13065641224159E-09", "module": "B2"}, {"value": "0", "module": "C1"}, {"value": "4.00824468942012E-09", "module": "C2", "scenario": "S0"}, {"value": "4.00824468942012E-09", "module": "C2", "scenario": "S1"}, {"value": "4.00824468942012E-09", "module": "C2", "scenario": "S2"}, {"value": "1.29843168465028E-09", "module": "C3", "scenario": "S0"}, {"value": "3.24607921162571E-09", "module": "C3", "scenario": "S1"}, {"value": "5.52256007129401E-09", "module": "C4", "scenario": "S0"}, {"value": "9.20426678549002E-09", "module": "C4", "scenario": "S2"}, {"value": "-1.34688733375582E-07", "module": "D", "scenario": "S0"}, {"value": "-2.66604256098356E-07", "module": "D", "scenario": "S1"}, {"value": "-4.67450515603995E-08", "module": "D", "scenario": "S2"}]}}, {"referenceToLCIAMethodDataSet": {"shortDescription": [{"value": "Acidification potential of land and water (AP)", "lang": "en"}, {"value": "Versauerungspotenzial von Boden und Wasser (AP)", "lang": "de"}], "type": "LCIA method data set", "refObjectId": "b5c611c6-def3-11e6-bf01-fe55135034f3", "uri": "../lciamethods/b5c611c6-def3-11e6-bf01-fe55135034f3.xml"}, "other": {"anies": [{"name": "referenceToUnitGroupDataSet", "value": {"shortDescription": [{"value": "mol H^(+)-Äq.", "lang": "en"}], "type": "unit group data set", "refObjectId": "42e089ac-92bf-4bf2-8ca1-5fc40d18f2ed", "uri": "../unitgroups/42e089ac-92bf-4bf2-8ca1-5fc40d18f2ed.xml"}}, {"value": "0.00900665436677184", "module": "A1-A3"}, {"value": "0.00176378919901186", "module": "A4"}, {"value": "0.00337194287782784", "module": "A5"}, {"value": "0.000561201975157516", "module": "B2"}, {"value": "0", "module": "C1"}, {"value": "8.77699950772103E-05", "module": "C2", "scenario": "S0"}, {"value": "8.77699950772103E-05", "module": "C2", "scenario": "S1"}, {"value": "8.77699950772103E-05", "module": "C2", "scenario": "S2"}, {"value": "0.000168124453924097", "module": "C3", "scenario": "S0"}, {"value": "0.000420311134810242", "module": "C3", "scenario": "S1"}, {"value": "0.000145476453556049", "module": "C4", "scenario": "S0"}, {"value": "0.000242460755926749", "module": "C4", "scenario": "S2"}, {"value": "-0.00954720630145619", "module": "D", "scenario": "S0"}, {"value": "-0.0191092258160979", "module": "D", "scenario": "S1"}, {"value": "-0.00317252662502838", "module": "D", "scenario": "S2"}]}}, {"referenceToLCIAMethodDataSet": {"shortDescription": [{"value": "Eutrophication potential aquatic freshwater (EP-freshwater)", "lang": "en"}, {"value": "Eutrophierungspotenzial Süßwasser (EP-freshwater)", "lang": "de"}], "type": "LCIA method data set", "refObjectId": "b53ec18f-7377-4ad3-86eb-cc3f4f276b2b", "uri": "../lciamethods/b53ec18f-7377-4ad3-86eb-cc3f4f276b2b.xml"}, "other": {"anies": [{"name": "referenceToUnitGroupDataSet", "value": {"shortDescription": [{"value": "kg PO_(4)-Äq.", "lang": "en"}], "type": "unit group data set", "refObjectId": "0429039d-a61d-4590-ba67-aa4a20a810a1", "uri": "../unitgroups/0429039d-a61d-4590-ba67-aa4a20a810a1.xml"}}, {"value": "0.00040083237442959", "module": "A1-A3"}, {"value": "1.62100366824342E-05", "module": "A4"}, {"value": "0.000118477103215843", "module": "A5"}, {"value": "6.28893139422716E-05", "module": "B2"}, {"value": "0", "module": "C1"}, {"value": "1.37797475849459E-06", "module": "C2", "scenario": "S0"}, {"value": "1.37797475849459E-06", "module": "C2", "scenario": "S1"}, {"value": "1.37797475849459E-06", "module": "C2", "scenario": "S2"}, {"value": "6.95206412428948E-06", "module": "C3", "scenario": "S0"}, {"value": "1.73801603107237E-05", "module": "C3", "scenario": "S1"}, {"value": "4.04446418530759E-06", "module": "C4", "scenario": "S0"}, {"value": "6.74077364217931E-06", "module": "C4", "scenario": "S2"}, {"value": "-0.00127119477878834", "module": "D", "scenario": "S0"}, {"value": "-0.00287401401475424", "module": "D", "scenario": "S1"}, {"value": "-0.000202648621477743", "module": "D", "scenario": "S2"}]}}, {"referenceToLCIAMethodDataSet": {"shortDescription": [{"value": "Eutrophication potential aquatic marine (EP-marine)", "lang": "en"}, {"value": "Eutrophierungspotenzial Salzwasser (EP-marine)", "lang": "de"}], "type": "LCIA method data set", "refObjectId": "b5c619fa-def3-11e6-bf01-fe55135034f3", "uri": "../lciamethods/b5c619fa-def3-11e6-bf01-fe55135034f3.xml"}, "other": {"anies": [{"name": "referenceToUnitGroupDataSet", "value": {"shortDescription": [{"value": "kg N-Äq.", "lang": "en"}], "type": "unit group data set", "refObjectId": "d05bb823-ecdf-4686-8c40-bf1d9257859f", "uri": "../unitgroups/d05bb823-ecdf-4686-8c40-bf1d9257859f.xml"}}, {"value": "0.00183269590280261", "module": "A1-A3"}, {"value": "0.000346999892785203", "module": "A4"}, {"value": "0.00030486312794178", "module": "A5"}, {"value": "0.000143289268988061", "module": "B2"}, {"value": "0", "module": "C1"}, {"value": "2.9741503962041E-05", "module": "C2", "scenario": "S0"}, {"value": "2.9741503962041E-05", "module": "C2", "scenario": "S1"}, {"value": "2.9741503962041E-05", "module": "C2", "scenario": "S2"}, {"value": "8.73530461403608E-05", "module": "C3", "scenario": "S0"}, {"value": "0.000218382615350902", "module": "C3", "scenario": "S1"}, {"value": "0.000577574887797612", "module": "C4", "scenario": "S0"}, {"value": "0.00096262481299602", "module": "C4", "scenario": "S2"}, {"value": "-0.00177821992195061", "module": "D", "scenario": "S0"}, {"value": "-0.00334002308288011", "module": "D", "scenario": "S1"}, {"value": "-0.000737017814664274", "module": "D", "scenario": "S2"}]}}, {"referenceToLCIAMethodDataSet": {"shortDescription": [{"value": "Eutrophication potential terrestrial (EP-terrestrial)", "lang": "en"}, {"value": "Eutrophierungspotenzial Land (EP-terrestrial)", "lang": "de"}], "type": "LCIA method data set", "refObjectId": "b5c614d2-def3-11e6-bf01-fe55135034f3", "uri": "../lciamethods/b5c614d2-def3-11e6-bf01-fe55135034f3.xml"}, "other": {"anies": [{"name": "referenceToUnitGroupDataSet", "value": {"shortDescription": [{"value": "mol N-Äq.", "lang": "en"}], "type": "unit group data set", "refObjectId": "71b4d617-0ec9-4d3f-b65e-e438940c2401", "uri": "../unitgroups/71b4d617-0ec9-4d3f-b65e-e438940c2401.xml"}}, {"value": "0.0217979182212917", "module": "A1-A3"}, {"value": "0.00385251592710664", "module": "A4"}, {"value": "0.00306592245497337", "module": "A5"}, {"value": "0.00110615697951757", "module": "B2"}, {"value": "0", "module": "C1"}, {"value": "0.000325309010398607", "module": "C2", "scenario": "S0"}, {"value": "0.000325309010398607", "module": "C2", "scenario": "S1"}, {"value": "0.000325309010398607", "module": "C2", "scenario": "S2"}, {"value": "0.000841428447596908", "module": "C3", "scenario": "S0"}, {"value": "0.00210357111899227", "module": "C3", "scenario": "S1"}, {"value": "0.000518880140195027", "module": "C4", "scenario": "S0"}, {"value": "0.000864800233658379", "module": "C4", "scenario": "S2"}, {"value": "-0.0188975108694265", "module": "D", "scenario": "S0"}, {"value": "-0.0352959025870136", "module": "D", "scenario": "S1"}, {"value": "-0.00796524972436844", "module": "D", "scenario": "S2"}]}}, {"referenceToLCIAMethodDataSet": {"shortDescription": [{"value": "Formation potential of tropospheric ozone photochemical oxidants (POCP)", "lang": "en"}, {"value": "Bildungspotential für troposphärisches Ozon (POCP)", "lang": "de"}], "type": "LCIA method data set", "refObjectId": "b5c610fe-def3-11e6-bf01-fe55135034f3", "uri": "../lciamethods/b5c610fe-def3-11e6-bf01-fe55135034f3.xml"}, "other": {"anies": [{"name": "referenceToUnitGroupDataSet", "value": {"shortDescription": [{"value": "kg NMVOC-Äq.", "lang": "en"}], "type": "unit group data set", "refObjectId": "d27c25f8-fbc1-44c6-b47b-4adbae4199c6", "uri": "../unitgroups/d27c25f8-fbc1-44c6-b47b-4adbae4199c6.xml"}}, {"value": "0.00625285129956354", "module": "A1-A3"}, {"value": "0.001092763246649", "module": "A4"}, {"value": "0.00107865447340974", "module": "A5"}, {"value": "0.000382852536822664", "module": "B2"}, {"value": "0", "module": "C1"}, {"value": "9.23204679182261E-05", "module": "C2", "scenario": "S0"}, {"value": "9.23204679182261E-05", "module": "C2", "scenario": "S1"}, {"value": "9.23204679182261E-05", "module": "C2", "scenario": "S2"}, {"value": "0.000205935743768034", "module": "C3", "scenario": "S0"}, {"value": "0.000514839359420085", "module": "C3", "scenario": "S1"}, {"value": "0.000186348744835593", "module": "C4", "scenario": "S0"}, {"value": "0.000310581241392655", "module": "C4", "scenario": "S2"}, {"value": "-0.00473824450761499", "module": "D", "scenario": "S0"}, {"value": "-0.00838188174430971", "module": "D", "scenario": "S1"}, {"value": "-0.00230915301648517", "module": "D", "scenario": "S2"}]}}, {"referenceToLCIAMethodDataSet": {"shortDescription": [{"value": "Abiotic depletion potential for non fossil resources (ADPE)", "lang": "en"}, {"value": "Potenzial für den abiotischen Abbau nicht fossiler Ressourcen (ADPE)", "lang": "de"}], "type": "LCIA method data set", "refObjectId": "b2ad6494-c78d-11e6-9d9d-cec0c932ce01", "uri": "../lciamethods/b2ad6494-c78d-11e6-9d9d-cec0c932ce01.xml"}, "other": {"anies": [{"name": "referenceToUnitGroupDataSet", "value": {"shortDescription": [{"value": "kg Sb-Äq.", "lang": "en"}], "type": "unit group data set", "refObjectId": "54ccd2d9-a32a-4fc2-923d-f2c8c93e89d4", "uri": "../unitgroups/54ccd2d9-a32a-4fc2-923d-f2c8c93e89d4.xml"}}, {"value": "3.8062008273361E-06", "module": "A1-A3"}, {"value": "3.18569967915573E-07", "module": "A4"}, {"value": "1.41840671112156E-06", "module": "A5"}, {"value": "2.69841294473659E-07", "module": "B2"}, {"value": "0", "module": "C1"}, {"value": "4.85082205502451E-08", "module": "C2", "scenario": "S0"}, {"value": "4.85082205502451E-08", "module": "C2", "scenario": "S1"}, {"value": "4.85082205502451E-08", "module": "C2", "scenario": "S2"}, {"value": "2.31749356610255E-08", "module": "C3", "scenario": "S0"}, {"value": "5.79373391525638E-08", "module": "C3", "scenario": "S1"}, {"value": "2.30564378446667E-08", "module": "C4", "scenario": "S0"}, {"value": "3.84273964077778E-08", "module": "C4", "scenario": "S2"}, {"value": "-1.77348733910671E-06", "module": "D", "scenario": "S0"}, {"value": "-2.60973145389276E-06", "module": "D", "scenario": "S1"}, {"value": "-1.21599126258267E-06", "module": "D", "scenario": "S2"}]}}, {"referenceToLCIAMethodDataSet": {"shortDescription": [{"value": "Abiotic depletion potential for fossil resources (ADPF)", "lang": "en"}, {"value": "Potenzial für den abiotischen Abbau fossiler Brennstoffe (ADPF)", "lang": "de"}], "type": "LCIA method data set", "refObjectId": "b2ad6110-c78d-11e6-9d9d-cec0c932ce01", "uri": "../lciamethods/b2ad6110-c78d-11e6-9d9d-cec0c932ce01.xml"}, "other": {"anies": [{"name": "referenceToUnitGroupDataSet", "value": {"shortDescription": [{"value": "MJ", "lang": "en"}], "type": "unit group data set", "refObjectId": "93a60a57-a3c8-11da-a746-0800200c9a66", "uri": "../unitgroups/93a60a57-a3c8-11da-a746-0800200c9a66.xml"}}, {"value": "22.9597089883658", "module": "A1-A3"}, {"value": "2.38920062908817", "module": "A4"}, {"value": "4.67922584159311", "module": "A5"}, {"value": "2.36134941481966", "module": "B2"}, {"value": "0", "module": "C1"}, {"value": "0.265525201678624", "module": "C2", "scenario": "S0"}, {"value": "0.265525201678624", "module": "C2", "scenario": "S1"}, {"value": "0.265525201678624", "module": "C2", "scenario": "S2"}, {"value": "0.136091016021077", "module": "C3", "scenario": "S0"}, {"value": "0.340227540052693", "module": "C3", "scenario": "S1"}, {"value": "0.417079141582873", "module": "C4", "scenario": "S0"}, {"value": "0.695131902638121", "module": "C4", "scenario": "S2"}, {"value": "-29.2879618394566", "module": "D", "scenario": "S0"}, {"value": "-61.3388184236338", "module": "D", "scenario": "S1"}, {"value": "-7.92072411667186", "module": "D", "scenario": "S2"}]}}, {"referenceToLCIAMethodDataSet": {"shortDescription": [{"value": "Water use (WDP)", "lang": "en"}, {"value": "Wassernutzung (WDP)", "lang": "de"}], "type": "LCIA method data set", "refObjectId": "b2ad66ce-c78d-11e6-9d9d-cec0c932ce01", "uri": "../lciamethods/b2ad66ce-c78d-11e6-9d9d-cec0c932ce01.xml"}, "other": {"anies": [{"name": "referenceToUnitGroupDataSet", "value": {"shortDescription": [{"value": "m^(3) world-Äq. deprived", "lang": "en"}], "type": "unit group data set", "refObjectId": "6ae2df01-888e-46c8-b17d-49fa3869b476", "uri": "../unitgroups/6ae2df01-888e-46c8-b17d-49fa3869b476.xml"}}, {"value": "1.56413963345027", "module": "A1-A3"}, {"value": "0.0163268750831968", "module": "A4"}, {"value": "0.280172864610155", "module": "A5"}, {"value": "0.0847669801806838", "module": "B2"}, {"value": "0", "module": "C1"}, {"value": "0.0018340601204069", "module": "C2", "scenario": "S0"}, {"value": "0.0018340601204069", "module": "C2", "scenario": "S1"}, {"value": "0.0018340601204069", "module": "C2", "scenario": "S2"}, {"value": "-0.00935899749629908", "module": "C3", "scenario": "S0"}, {"value": "-0.0233974937407477", "module": "C3", "scenario": "S1"}, {"value": "0.0178855101993324", "module": "C4", "scenario": "S0"}, {"value": "0.029809183665554", "module": "C4", "scenario": "S2"}, {"value": "-0.971808475085773", "module": "D", "scenario": "S0"}, {"value": "-1.42269038367494", "module": "D", "scenario": "S1"}, {"value": "-0.671220536026328", "module": "D", "scenario": "S2"}]}}, {"referenceToLCIAMethodDataSet": {"shortDescription": [{"value": "Incidence of disease due to PM emissions (PM)", "lang": "en"}, {"value": "Auftreten von Krankheiten aufgrund von Feinstaubemissionen (PM)", "lang": "de"}], "type": "LCIA method data set", "refObjectId": "b5c602c6-def3-11e6-bf01-fe55135034f3", "uri": "../lciamethods/b5c602c6-def3-11e6-bf01-fe55135034f3.xml"}, "other": {"anies": [{"name": "referenceToUnitGroupDataSet", "value": {"shortDescription": [{"value": "Disease incidence", "lang": "en"}], "type": "unit group data set", "refObjectId": "3883559b-648f-4afc-8ba2-0bd24f3affa3", "uri": "../unitgroups/3883559b-648f-4afc-8ba2-0bd24f3affa3.xml"}}, {"module": "A1-A3"}, {"module": "A4"}, {"module": "A5"}, {"module": "B2"}, {"module": "C1"}, {"module": "C2", "scenario": "S0"}, {"module": "C2", "scenario": "S1"}, {"module": "C2", "scenario": "S2"}, {"module": "C3", "scenario": "S0"}, {"module": "C3", "scenario": "S1"}, {"module": "C4", "scenario": "S0"}, {"module": "C4", "scenario": "S2"}, {"module": "D", "scenario": "S0"}, {"module": "D", "scenario": "S1"}, {"module": "D", "scenario": "S2"}]}}, {"referenceToLCIAMethodDataSet": {"shortDescription": [{"value": "Human exposure efficiency relative to U235 (IR)", "lang": "en"}, {"value": "Wirkung durch Exposition des Menschen mit U235 (IR)", "lang": "de"}], "type": "LCIA method data set", "refObjectId": "b5c632be-def3-11e6-bf01-fe55135034f3", "uri": "../lciamethods/b5c632be-def3-11e6-bf01-fe55135034f3.xml"}, "other": {"anies": [{"name": "referenceToUnitGroupDataSet", "value": {"shortDescription": [{"value": "kBq U235-Äq.", "lang": "en"}], "type": "unit group data set", "refObjectId": "456b05bf-1415-44a9-9993-02452f554c09", "uri": "../unitgroups/456b05bf-1415-44a9-9993-02452f554c09.xml"}}, {"module": "A1-A3"}, {"module": "A4"}, {"module": "A5"}, {"module": "B2"}, {"module": "C1"}, {"module": "C2", "scenario": "S0"}, {"module": "C2", "scenario": "S1"}, {"module": "C2", "scenario": "S2"}, {"module": "C3", "scenario": "S0"}, {"module": "C3", "scenario": "S1"}, {"module": "C4", "scenario": "S0"}, {"module": "C4", "scenario": "S2"}, {"module": "D", "scenario": "S0"}, {"module": "D", "scenario": "S1"}, {"module": "D", "scenario": "S2"}]}}, {"referenceToLCIAMethodDataSet": {"shortDescription": [{"value": "Comparative toxic unit for ecosystems (ETP-fw)", "lang": "en"}, {"value": "Toxizitätsvergleichseinheit für Ökosysteme (ETP-fw)", "lang": "de"}], "type": "LCIA method data set", "refObjectId": "ee1082d1-b0f7-43ca-a1f0-21e2a4a74511", "uri": "../lciamethods/ee1082d1-b0f7-43ca-a1f0-21e2a4a74511.xml"}, "other": {"anies": [{"name": "referenceToUnitGroupDataSet", "value": {"shortDescription": [{"value": "CTUe", "lang": "en"}], "type": "unit group data set", "refObjectId": "aa959ded-f1eb-4efb-9c5c-2d60be36b3e6", "uri": "../unitgroups/aa959ded-f1eb-4efb-9c5c-2d60be36b3e6.xml"}}, {"module": "A1-A3"}, {"module": "A4"}, {"module": "A5"}, {"module": "B2"}, {"module": "C1"}, {"module": "C2", "scenario": "S0"}, {"module": "C2", "scenario": "S1"}, {"module": "C2", "scenario": "S2"}, {"module": "C3", "scenario": "S0"}, {"module": "C3", "scenario": "S1"}, {"module": "C4", "scenario": "S0"}, {"module": "C4", "scenario": "S2"}, {"module": "D", "scenario": "S0"}, {"module": "D", "scenario": "S1"}, {"module": "D", "scenario": "S2"}]}}, {"referenceToLCIAMethodDataSet": {"shortDescription": [{"value": "Comparative toxic unit for humans (carcinogenic) (HTP-c)", "lang": "en"}, {"value": "Toxizitätsvergleichseinheit für Menschen (krebserregend) (HTP-c)", "lang": "de"}], "type": "LCIA method data set", "refObjectId": "2299222a-bbd8-474f-9d4f-4dd1f18aea7c", "uri": "../lciamethods/2299222a-bbd8-474f-9d4f-4dd1f18aea7c.xml"}, "other": {"anies": [{"name": "referenceToUnitGroupDataSet", "value": {"shortDescription": [{"value": "CTUh", "lang": "en"}], "type": "unit group data set", "refObjectId": "d4c9523e-2d7e-49fd-8469-998f547d3a70", "uri": "../unitgroups/d4c9523e-2d7e-49fd-8469-998f547d3a70.xml"}}, {"module": "A1-A3"}, {"module": "A4"}, {"module": "A5"}, {"module": "B2"}, {"module": "C1"}, {"module": "C2", "scenario": "S0"}, {"module": "C2", "scenario": "S1"}, {"module": "C2", "scenario": "S2"}, {"module": "C3", "scenario": "S0"}, {"module": "C3", "scenario": "S1"}, {"module": "C4", "scenario": "S0"}, {"module": "C4", "scenario": "S2"}, {"module": "D", "scenario": "S0"}, {"module": "D", "scenario": "S1"}, {"module": "D", "scenario": "S2"}]}}, {"referenceToLCIAMethodDataSet": {"shortDescription": [{"value": "Comparative toxic unit for humans (noncarcinogenic) (HTP-nc)", "lang": "en"}, {"value": "Toxizitätsvergleichseinheit für Menschen (nicht krebserregend) (HTP-nc)", "lang": "de"}], "type": "LCIA method data set", "refObjectId": "3af763a5-b7a1-48c9-9cee-1f223481fcef", "uri": "../lciamethods/3af763a5-b7a1-48c9-9cee-1f223481fcef.xml"}, "other": {"anies": [{"name": "referenceToUnitGroupDataSet", "value": {"shortDescription": [{"value": "CTUh", "lang": "en"}], "type": "unit group data set", "refObjectId": "d4c9523e-2d7e-49fd-8469-998f547d3a70", "uri": "../unitgroups/d4c9523e-2d7e-49fd-8469-998f547d3a70.xml"}}, {"module": "A1-A3"}, {"module": "A4"}, {"module": "A5"}, {"module": "B2"}, {"module": "C1"}, {"module": "C2", "scenario": "S0"}, {"module": "C2", "scenario": "S1"}, {"module": "C2", "scenario": "S2"}, {"module": "C3", "scenario": "S0"}, {"module": "C3", "scenario": "S1"}, {"module": "C4", "scenario": "S0"}, {"module": "C4", "scenario": "S2"}, {"module": "D", "scenario": "S0"}, {"module": "D", "scenario": "S1"}, {"module": "D", "scenario": "S2"}]}}, {"referenceToLCIAMethodDataSet": {"shortDescription": [{"value": "Soil quality index (SQP)", "lang": "en"}, {"value": "Bodenqualitätsindex (SQP)", "lang": "de"}], "type": "LCIA method data set", "refObjectId": "b2ad6890-c78d-11e6-9d9d-cec0c932ce01", "uri": "../lciamethods/b2ad6890-c78d-11e6-9d9d-cec0c932ce01.xml"}, "other": {"anies": [{"name": "referenceToUnitGroupDataSet", "value": {"shortDescription": [{"value": "SQP", "lang": "en"}], "type": "unit group data set", "refObjectId": "f130951c-e67f-4f7f-8dd4-665de3974e18", "uri": "../unitgroups/f130951c-e67f-4f7f-8dd4-665de3974e18.xml"}}, {"module": "A1-A3"}, {"module": "A4"}, {"module": "A5"}, {"module": "B2"}, {"module": "C1"}, {"module": "C2", "scenario": "S0"}, {"module": "C2", "scenario": "S1"}, {"module": "C2", "scenario": "S2"}, {"module": "C3", "scenario": "S0"}, {"module": "C3", "scenario": "S1"}, {"module": "C4", "scenario": "S0"}, {"module": "C4", "scenario": "S2"}, {"module": "D", "scenario": "S0"}, {"module": "D", "scenario": "S1"}, {"module": "D", "scenario": "S2"}]}}]}, "otherAttributes": {"{http://www.indata.network/EPD/2019}epd-version": "1.2"}, "version": "1.1", "locations": "../ILCDLocations.xml"}