{"processInformation": {"dataSetInformation": {"UUID": "83de9d28-84bf-43e1-b893-d8aedbfebe16", "name": {"baseName": [{"value": "UZIN RenoTop PLUS Flooring System", "lang": "en"}, {"value": "UZIN RenoTop PLUS Bodenbelag", "lang": "de"}]}, "classificationInformation": {"classification": [{"class": [{"value": "Holz", "level": 0, "classId": "3"}, {"value": "Holzböden", "level": 1, "classId": "3.3"}, {"value": "Mehrschichtig modulare Bodenbeläge", "level": 2, "classId": "3.3.04"}], "name": "OEKOBAU.DAT"}]}, "generalComment": [{"value": "This EPD is based on the life cycle assessment of the UZIN RenoTop PLUS flooring system produced by a partner company of Uzin Utz SE. The declaration holder is liable for the underlying information and evidence. Kiwa-Ecobility Experts is not liable for manufacturer information, life cycle assessment data and evidence.", "lang": "en"}], "other": {"anies": [{"scenario": [{"description": [{"value": "For data protection reasons, the assumptions made and data used are only explained in the background report accompanying this EPD. For the transport to the construction site in module A4, a scenario with a distance of 286 km and the environmental profile \"market group for transport, freight, lorry, unspecified {GLO}\" from Ecoinvent 3.6 was used. No auxiliary or operating materials or energy were taken into account when installing the product in module A5, as only human muscle power is required for the installation. There are no direct emissions into the ambient air, soil or water. But there is packaging waste in the form of protective film, which is removed from the adhesive surfaces, and a Euro pallet, which was used for transport. As a conservative approach, an additional 3 % installation waste was assumed. For disposal, a waste scenario for \"MDF\" based on the NMD waste scenario ID 36 from the Netherlands was adapted and used for Germany. Here, 5 % landfilling and 95 % incineration were assumed. For the distance to waste treatment, 100 km for landfilling and 150 km for incineration were used with \"market group for transport, freight, lorry, unspecified {GLO}\" (from Ecoinvent 3.6). The energy saving (credit) from incineration was adjusted for the German market. For the landfill loads, \"99% Waste wood, untreated and 1% Waste paint {EU}| treatment of, sanitary landfill\" was used and for the incineration \"Waste building wood, chrome preserved {CH}| treatment of, municipal incineration\"."}], "name": "Standard Scenario", "default": true}]}, "<ns11:modules xmlns:ns11=\"http://openlca.org/epd_ilcd\" xmlns=\"http://lca.jrc.it/ILCD/Process\" xmlns:c=\"http://lca.jrc.it/ILCD/Contact\" xmlns:common=\"http://lca.jrc.it/ILCD/Common\" xmlns:epd=\"http://www.iai.kit.edu/EPD/2013\" xmlns:epd2=\"http://www.indata.network/EPD/2019\" xmlns:f=\"http://lca.jrc.it/ILCD/Flow\" xmlns:fp=\"http://lca.jrc.it/ILCD/FlowProperty\" xmlns:m=\"http://lca.jrc.it/ILCD/LCIAMethod\" xmlns:ns9=\"http://www.okworx.com/ILCD/Extensions/2018/Profile\" xmlns:s=\"http://lca.jrc.it/ILCD/Source\" xmlns:u=\"http://lca.jrc.it/ILCD/UnitGroup\" name=\"A1\" scenario=\"Standard Scenario\"/>", "<ns11:modules xmlns:ns11=\"http://openlca.org/epd_ilcd\" xmlns=\"http://lca.jrc.it/ILCD/Process\" xmlns:c=\"http://lca.jrc.it/ILCD/Contact\" xmlns:common=\"http://lca.jrc.it/ILCD/Common\" xmlns:epd=\"http://www.iai.kit.edu/EPD/2013\" xmlns:epd2=\"http://www.indata.network/EPD/2019\" xmlns:f=\"http://lca.jrc.it/ILCD/Flow\" xmlns:fp=\"http://lca.jrc.it/ILCD/FlowProperty\" xmlns:m=\"http://lca.jrc.it/ILCD/LCIAMethod\" xmlns:ns9=\"http://www.okworx.com/ILCD/Extensions/2018/Profile\" xmlns:s=\"http://lca.jrc.it/ILCD/Source\" xmlns:u=\"http://lca.jrc.it/ILCD/UnitGroup\" name=\"A2\" scenario=\"Standard Scenario\"/>", "<ns11:modules xmlns:ns11=\"http://openlca.org/epd_ilcd\" xmlns=\"http://lca.jrc.it/ILCD/Process\" xmlns:c=\"http://lca.jrc.it/ILCD/Contact\" xmlns:common=\"http://lca.jrc.it/ILCD/Common\" xmlns:epd=\"http://www.iai.kit.edu/EPD/2013\" xmlns:epd2=\"http://www.indata.network/EPD/2019\" xmlns:f=\"http://lca.jrc.it/ILCD/Flow\" xmlns:fp=\"http://lca.jrc.it/ILCD/FlowProperty\" xmlns:m=\"http://lca.jrc.it/ILCD/LCIAMethod\" xmlns:ns9=\"http://www.okworx.com/ILCD/Extensions/2018/Profile\" xmlns:s=\"http://lca.jrc.it/ILCD/Source\" xmlns:u=\"http://lca.jrc.it/ILCD/UnitGroup\" name=\"A3\" scenario=\"Standard Scenario\"/>", "<ns11:modules xmlns:ns11=\"http://openlca.org/epd_ilcd\" xmlns=\"http://lca.jrc.it/ILCD/Process\" xmlns:c=\"http://lca.jrc.it/ILCD/Contact\" xmlns:common=\"http://lca.jrc.it/ILCD/Common\" xmlns:epd=\"http://www.iai.kit.edu/EPD/2013\" xmlns:epd2=\"http://www.indata.network/EPD/2019\" xmlns:f=\"http://lca.jrc.it/ILCD/Flow\" xmlns:fp=\"http://lca.jrc.it/ILCD/FlowProperty\" xmlns:m=\"http://lca.jrc.it/ILCD/LCIAMethod\" xmlns:ns9=\"http://www.okworx.com/ILCD/Extensions/2018/Profile\" xmlns:s=\"http://lca.jrc.it/ILCD/Source\" xmlns:u=\"http://lca.jrc.it/ILCD/UnitGroup\" name=\"A4\" scenario=\"Standard Scenario\"/>", "<ns11:modules xmlns:ns11=\"http://openlca.org/epd_ilcd\" xmlns=\"http://lca.jrc.it/ILCD/Process\" xmlns:c=\"http://lca.jrc.it/ILCD/Contact\" xmlns:common=\"http://lca.jrc.it/ILCD/Common\" xmlns:epd=\"http://www.iai.kit.edu/EPD/2013\" xmlns:epd2=\"http://www.indata.network/EPD/2019\" xmlns:f=\"http://lca.jrc.it/ILCD/Flow\" xmlns:fp=\"http://lca.jrc.it/ILCD/FlowProperty\" xmlns:m=\"http://lca.jrc.it/ILCD/LCIAMethod\" xmlns:ns9=\"http://www.okworx.com/ILCD/Extensions/2018/Profile\" xmlns:s=\"http://lca.jrc.it/ILCD/Source\" xmlns:u=\"http://lca.jrc.it/ILCD/UnitGroup\" name=\"A5\" scenario=\"Standard Scenario\"/>", "<ns11:modules xmlns:ns11=\"http://openlca.org/epd_ilcd\" xmlns=\"http://lca.jrc.it/ILCD/Process\" xmlns:c=\"http://lca.jrc.it/ILCD/Contact\" xmlns:common=\"http://lca.jrc.it/ILCD/Common\" xmlns:epd=\"http://www.iai.kit.edu/EPD/2013\" xmlns:epd2=\"http://www.indata.network/EPD/2019\" xmlns:f=\"http://lca.jrc.it/ILCD/Flow\" xmlns:fp=\"http://lca.jrc.it/ILCD/FlowProperty\" xmlns:m=\"http://lca.jrc.it/ILCD/LCIAMethod\" xmlns:ns9=\"http://www.okworx.com/ILCD/Extensions/2018/Profile\" xmlns:s=\"http://lca.jrc.it/ILCD/Source\" xmlns:u=\"http://lca.jrc.it/ILCD/UnitGroup\" name=\"C1\" scenario=\"Standard Scenario\"/>", "<ns11:modules xmlns:ns11=\"http://openlca.org/epd_ilcd\" xmlns=\"http://lca.jrc.it/ILCD/Process\" xmlns:c=\"http://lca.jrc.it/ILCD/Contact\" xmlns:common=\"http://lca.jrc.it/ILCD/Common\" xmlns:epd=\"http://www.iai.kit.edu/EPD/2013\" xmlns:epd2=\"http://www.indata.network/EPD/2019\" xmlns:f=\"http://lca.jrc.it/ILCD/Flow\" xmlns:fp=\"http://lca.jrc.it/ILCD/FlowProperty\" xmlns:m=\"http://lca.jrc.it/ILCD/LCIAMethod\" xmlns:ns9=\"http://www.okworx.com/ILCD/Extensions/2018/Profile\" xmlns:s=\"http://lca.jrc.it/ILCD/Source\" xmlns:u=\"http://lca.jrc.it/ILCD/UnitGroup\" name=\"C2\" scenario=\"Standard Scenario\"/>", "<ns11:modules xmlns:ns11=\"http://openlca.org/epd_ilcd\" xmlns=\"http://lca.jrc.it/ILCD/Process\" xmlns:c=\"http://lca.jrc.it/ILCD/Contact\" xmlns:common=\"http://lca.jrc.it/ILCD/Common\" xmlns:epd=\"http://www.iai.kit.edu/EPD/2013\" xmlns:epd2=\"http://www.indata.network/EPD/2019\" xmlns:f=\"http://lca.jrc.it/ILCD/Flow\" xmlns:fp=\"http://lca.jrc.it/ILCD/FlowProperty\" xmlns:m=\"http://lca.jrc.it/ILCD/LCIAMethod\" xmlns:ns9=\"http://www.okworx.com/ILCD/Extensions/2018/Profile\" xmlns:s=\"http://lca.jrc.it/ILCD/Source\" xmlns:u=\"http://lca.jrc.it/ILCD/UnitGroup\" name=\"C3\" scenario=\"Standard Scenario\"/>", "<ns11:modules xmlns:ns11=\"http://openlca.org/epd_ilcd\" xmlns=\"http://lca.jrc.it/ILCD/Process\" xmlns:c=\"http://lca.jrc.it/ILCD/Contact\" xmlns:common=\"http://lca.jrc.it/ILCD/Common\" xmlns:epd=\"http://www.iai.kit.edu/EPD/2013\" xmlns:epd2=\"http://www.indata.network/EPD/2019\" xmlns:f=\"http://lca.jrc.it/ILCD/Flow\" xmlns:fp=\"http://lca.jrc.it/ILCD/FlowProperty\" xmlns:m=\"http://lca.jrc.it/ILCD/LCIAMethod\" xmlns:ns9=\"http://www.okworx.com/ILCD/Extensions/2018/Profile\" xmlns:s=\"http://lca.jrc.it/ILCD/Source\" xmlns:u=\"http://lca.jrc.it/ILCD/UnitGroup\" name=\"C4\" scenario=\"Standard Scenario\"/>", "<ns11:modules xmlns:ns11=\"http://openlca.org/epd_ilcd\" xmlns=\"http://lca.jrc.it/ILCD/Process\" xmlns:c=\"http://lca.jrc.it/ILCD/Contact\" xmlns:common=\"http://lca.jrc.it/ILCD/Common\" xmlns:epd=\"http://www.iai.kit.edu/EPD/2013\" xmlns:epd2=\"http://www.indata.network/EPD/2019\" xmlns:f=\"http://lca.jrc.it/ILCD/Flow\" xmlns:fp=\"http://lca.jrc.it/ILCD/FlowProperty\" xmlns:m=\"http://lca.jrc.it/ILCD/LCIAMethod\" xmlns:ns9=\"http://www.okworx.com/ILCD/Extensions/2018/Profile\" xmlns:s=\"http://lca.jrc.it/ILCD/Source\" xmlns:u=\"http://lca.jrc.it/ILCD/UnitGroup\" name=\"D\" scenario=\"Standard Scenario\"/>"]}}, "quantitativeReference": {"referenceToReferenceFlow": [1], "type": "Reference flow(s)"}, "time": {"referenceYear": 2021, "dataSetValidUntil": 2027, "timeRepresentativenessDescription": [{"value": "All product- and process-specific data were collected for the operating year 2021 and are therefore up-to-date.", "lang": "en"}], "other": {"anies": [{"name": "publicationDateOfEPD", "value": 1668124800000}]}}, "geography": {"locationOfOperationSupplyOrProduction": {"location": "DE"}}, "technology": {"technologyDescriptionAndIncludedProcesses": [{"value": "UZIN RenoTop PLUS has been specially developed for objects with higher quality requirements and heavy loads due to high walking frequency and point loads. The subfloor system, consisting of bottom and top panels, in combination with a levelling layer with very high bulk density, bears these loads stably and reliably for years. Unnecessary loss of time that occurs when levelling with levelling compounds is avoided. Jum-pax® HD can be laid immediately on many problematic subfloors without tedious preparatory work. This saves a lot of time during renovations. The room is perfect, reliable and quickly in shape for the desired floor and the design ideas of your customers. The noise-reducing property has been tested in combination with vinyl and linoleum according to European standard EN-ISO 140-8 / 717-2. The floor was loaded with 23 kg / m². The improvement was achieved on a concrete floor with attached screed. On floating screed systems, the sound insulation of the floor covering is always dependent on the impact sound insulation of the existing screed. Due to its excellent stability, UZIN RenoTop PLUS is suitable as an underlay for 2nd/3rd layer prefabricated parquet. With a system height of only 10 mm and a load capacity of 4 kN point load, UZIN RenoTop PLUS is the most efficient dry screed with best impact sound reduction values of min 20 dB. UZIN RenoTop PLUS is manufactured by a partner company of Uzin Utz SE at De Bolder in Texel in the Netherlands (Reijer Keijserstraat 8, 1791 AX Den Burg - Texel). In this process, the individual layers (MDF etc.) are joined together with glue and then packed for transport to the place of use.\r\n", "lang": "en"}], "technologicalApplicability": [{"value": "UZIN RenoTop PLUS has been specially developed for objects with higher quality requirements and heavy loads due to high walking frequency and point loads. The subfloor system, consisting of bottom and top panels, in combination with a levelling layer with very high bulk density, bears these loads stably and reliably for years. Due to its excellent stability, UZIN RenoTop PLUS is suitable as an underlay for 2nd/3rd layer prefabricated parquet.", "lang": "en"}], "referenceToTechnologyFlowDiagrammOrPicture": [{"shortDescription": [{"value": "Flow Chart UZIN RenoTop PLUS", "lang": "en"}], "type": "source data set", "refObjectId": "f9bc91ff-7622-4063-a5fe-dfcd839c620e", "version": "00.00.002"}]}}, "modellingAndValidation": {"LCIMethodAndAllocation": {"typeOfDataSet": "EPD", "other": {"anies": [{"name": "subType", "value": "specific dataset"}]}}, "dataSourcesTreatmentAndRepresentativeness": {"referenceToDataSource": [{"shortDescription": [{"value": "ecoinvent database (general)", "lang": "en"}], "type": "source data set", "refObjectId": "b497a91f-e14b-4b69-8f28-f50eb1576766", "version": "00.03.002"}, {"shortDescription": [{"value": "ecoinvent 3.6 database", "lang": "en"}], "type": "source data set", "refObjectId": "766b9973-5ee8-48a2-8098-72c8e20b369f", "version": "00.00.001"}], "useAdviceForDataSet": [{"value": "UZIN RenoTop PLUS has been specially developed for objects with higher quality requirements and heavy loads due to high walking frequency and point loads. The subfloor system, consisting of bottom and top panels, in combination with a levelling layer with very high bulk density, bears these loads stably and reliably for years. Unnecessary loss of time that occurs when levelling with levelling compounds is avoided. Jum-pax® HD can be laid immediately on many problematic subfloors without tedious preparatory work. This saves a lot of time during renovations. The room is perfect, reliable and quickly in shape for the desired floor and the design ideas of your customers. The noise-reducing property has been tested in combination with vinyl and linoleum according to European standard EN-ISO 140-8 / 717-2. The floor was loaded with 23 kg / m². The improvement was achieved on a concrete floor with attached screed. On floating screed systems, the sound insulation of the floor covering is always dependent on the impact sound insulation of the existing screed. Due to its excellent stability, UZIN RenoTop PLUS is suitable as an underlay for 2nd/3rd layer prefabricated parquet. With a system height of only 10 mm and a load capacity of 4 kN point load, UZIN RenoTop PLUS is the most efficient dry screed with best impact sound reduction values of min 20 dB.", "lang": "en"}], "other": {"anies": [{"name": "referenceToOriginalEPD", "value": {"shortDescription": {"value": "EPD for UZIN RenoTop PLUS", "defaultValue": "EPD for UZIN RenoTop PLUS", "lstrings": [{"lang": "en", "value": "EPD for UZIN RenoTop PLUS"}]}, "version": {"version": 1, "majorVersion": 0, "minorVersion": 0, "subMinorVersion": 1, "zero": false, "versionString": "00.00.001"}, "type": "source data set", "uuid": {"uuid": "dcdd6ab0-e11e-478c-a826-30fd2f893ad9"}, "refObjectId": "dcdd6ab0-e11e-478c-a826-30fd2f893ad9", "versionAsString": "00.00.001", "resourceURLs": ["https://oekobaudat.de/OEKOBAU.DAT/resource/sources/dcdd6ab0-e11e-478c-a826-30fd2f893ad9/EPD-UzinUtz-306-EN.pdf?version=00.00.001"]}}]}}, "validation": {"review": [{"reviewDetails": [{"value": "Independent verification of the declaration and data according to EN ISO 14025:2011-10.", "lang": "en"}], "referenceToNameOfReviewerAndInstitution": [{"shortDescription": [{"value": "Julian Rickert (Third party verifier) ", "lang": "en"}], "type": "contact data set", "refObjectId": "c92a6ffe-7e89-41d2-8a14-e48cfbdd273c", "version": "00.00.001"}], "type": "Independent external review"}]}, "complianceDeclarations": {"compliance": [{"referenceToComplianceSystem": {"shortDescription": [{"value": "EN 15804+A2 (EF 3.0)", "lang": "de"}, {"value": "EN 15804+A2 (EF 3.0)", "lang": "en"}], "type": "source data set", "refObjectId": "c0016b33-8cf7-415c-ac6e-deba0d21440d", "version": "00.02.000"}}, {"referenceToComplianceSystem": {"shortDescription": [{"value": "ISO 14025", "lang": "en"}], "type": "source data set", "refObjectId": "4f2eb655-6e44-4874-a95a-e28f5442cd4d", "version": "00.00.001"}}]}}, "administrativeInformation": {"commissionerAndGoal": {"referenceToCommissioner": [{"shortDescription": [{"value": "Uzin Utz SE", "lang": "en"}], "type": "contact data set", "refObjectId": "7f4799c3-aa0f-4653-8846-ab4fe15c07cd", "version": "00.00.002"}]}, "dataGenerator": {"referenceToPersonOrEntityGeneratingTheDataSet": [{"shortDescription": [{"value": "Kiwa GmbH (Berlin)", "lang": "en"}], "type": "contact data set", "refObjectId": "3ea4a87a-3f88-4633-b7e7-1bbdd272be43", "version": "00.00.002"}]}, "dataEntryBy": {"timeStamp": 1745394102837, "referenceToDataSetFormat": [{"shortDescription": [{"value": "EPD Data Format Extensions v1.2", "lang": "en"}, {"value": "EPD-Datenformaterweiterungen v1.2", "lang": "de"}], "type": "source data set", "refObjectId": "a29449fd-aa2f-4de8-b5d7-4b06b43c6fde", "version": "00.01.000"}, {"shortDescription": [{"value": "ILCD format", "lang": "en"}], "type": "source data set", "refObjectId": "a97a0155-0234-4b87-b4ce-a45da52f2a40", "version": "01.00.000", "uri": "http://lca.jrc.ec.europa.eu/lcainfohub/sample_data/ilcd/sources/ILCD_Format_a97a0155-0234-4b87-b4ce-a45da52f2a40_01.00.000.xml"}], "referenceToPersonOrEntityEnteringTheData": {"shortDescription": [{"value": "Kiwa GmbH (Berlin)", "lang": "en"}], "type": "contact data set", "refObjectId": "3ea4a87a-3f88-4633-b7e7-1bbdd272be43", "version": "00.00.002"}}, "publicationAndOwnership": {"dataSetVersion": "00.00.018", "referenceToRegistrationAuthority": {"shortDescription": [{"value": "Kiwa-Ecobility Experts, Kiwa GmbH (Berlin)", "lang": "en"}], "type": "contact data set", "refObjectId": "eb52a9a8-9d0f-40ce-a5c9-7b78f5615e5a", "version": "00.00.002"}, "registrationNumber": "EPD-UzinUtz-306-EN", "referenceToOwnershipOfDataSet": {"shortDescription": [{"value": "Uzin Utz SE", "lang": "en"}], "type": "contact data set", "refObjectId": "7f4799c3-aa0f-4653-8846-ab4fe15c07cd", "version": "00.00.002"}, "copyright": true, "licenseType": "Free of charge for all users and uses", "accessRestrictions": [{"value": "None", "lang": "en"}], "other": {"anies": [{"name": "referenceToPublisher", "value": {"shortDescription": [{"value": "Kiwa-Ecobility Experts, Kiwa GmbH (Berlin)", "lang": "en"}], "type": "contact data set", "refObjectId": "eb52a9a8-9d0f-40ce-a5c9-7b78f5615e5a", "version": "00.00.002"}}]}}}, "exchanges": {"exchange": [{"dataSetInternalID": 1, "referenceToFlowDataSet": {"shortDescription": [{"value": "UZIN RenoTop PLUS", "lang": "en"}], "type": "flow data set", "refObjectId": "986ce59c-1d90-498a-b3e6-99b368b1459c", "version": "00.00.006"}, "meanAmount": 1.0, "resultingAmount": 1.0, "referenceFlow": true, "resultingflowAmount": 1.0, "flowProperties": [{"name": [{"lang": "de", "value": "Fläche"}, {"lang": "en", "value": "Area"}], "uuid": "93a60a56-a3c8-19da-a746-0800200c9a66", "referenceFlowProperty": true, "meanValue": 1.0, "referenceUnit": "qm", "unitGroupUUID": "c20a03d7-bd90-4569-bc94-66cfd364dfc8"}], "materialProperties": [{"name": "layer thickness", "value": "0.01", "unit": "m", "unitDescription": "meters"}, {"name": "grammage", "value": "6.45", "unit": "kg/m^2", "unitDescription": "kilograms per square meter"}], "typeOfFlow": "Product flow", "classification": {"classHierarchy": "Holz / Holzböden / Mehrschichtig modulare Bodenbeläge", "name": "OEKOBAU.DAT"}}, {"dataSetInternalID": 2, "referenceToFlowDataSet": {"shortDescription": [{"value": "Components for re-use (CRU)", "lang": "en"}, {"value": "Komponenten für die Wiederverwendung (CRU)", "lang": "de"}, {"value": "Componentes para su reutilización (CRU)", "lang": "es"}], "type": "flow data set", "refObjectId": "a2b32f97-3fc7-4af2-b209-525bc6426f33", "version": "30.00.000"}, "exchange direction": "OUTPUT", "meanAmount": 0.0, "other": {"anies": [{"value": "0.0", "module": "A1", "scenario": "Standard Scenario"}, {"value": "0.0", "module": "A2", "scenario": "Standard Scenario"}, {"value": "0.0", "module": "A3", "scenario": "Standard Scenario"}, {"value": "0.0", "module": "A4", "scenario": "Standard Scenario"}, {"value": "0.0", "module": "A5", "scenario": "Standard Scenario"}, {"value": "0.0", "module": "C1", "scenario": "Standard Scenario"}, {"value": "0.0", "module": "C2", "scenario": "Standard Scenario"}, {"value": "0.0", "module": "C3", "scenario": "Standard Scenario"}, {"value": "0.0", "module": "C4", "scenario": "Standard Scenario"}, {"value": "0.0", "module": "D", "scenario": "Standard Scenario"}, {"name": "referenceToUnitGroupDataSet", "value": {"shortDescription": [{"value": "kg"}], "type": "unit group data set", "refObjectId": "ad38d542-3fe9-439d-9b95-2f5f7752acaf", "uri": "../unitgroups/ad38d542-3fe9-439d-9b95-2f5f7752acaf"}}]}, "flowProperties": [], "typeOfFlow": "Other flow", "classification": {"classHierarchy": "Größen / Umweltliche Größen / EPD EN 15804 / LCI Indikatoren", "name": "GaBiCategories"}}, {"dataSetInternalID": 3, "referenceToFlowDataSet": {"shortDescription": [{"value": "Exported electrical energy (EEE)", "lang": "en"}, {"value": "Exportierte elektrische Energie (EEE)", "lang": "de"}, {"value": "Energía exportada electrica (EEE)", "lang": "es"}], "type": "flow data set", "refObjectId": "4da0c987-2b76-40d6-9e9e-82a017aaaf29", "version": "30.00.000"}, "exchange direction": "OUTPUT", "meanAmount": 0.0, "other": {"anies": [{"value": "0.0", "module": "A1", "scenario": "Standard Scenario"}, {"value": "0.0", "module": "A2", "scenario": "Standard Scenario"}, {"value": "-0.794", "module": "A3", "scenario": "Standard Scenario"}, {"value": "0.0", "module": "A4", "scenario": "Standard Scenario"}, {"value": "0.0", "module": "A5", "scenario": "Standard Scenario"}, {"value": "0.0", "module": "C1", "scenario": "Standard Scenario"}, {"value": "0.0", "module": "C2", "scenario": "Standard Scenario"}, {"value": "51.4", "module": "C3", "scenario": "Standard Scenario"}, {"value": "0.0", "module": "C4", "scenario": "Standard Scenario"}, {"value": "-27.3", "module": "D", "scenario": "Standard Scenario"}, {"name": "referenceToUnitGroupDataSet", "value": {"shortDescription": [{"value": "MJ"}], "type": "unit group data set", "refObjectId": "93a60a57-a3c8-11da-a746-0800200c9a66", "uri": "../unitgroups/93a60a57-a3c8-11da-a746-0800200c9a66"}}]}, "flowProperties": [], "typeOfFlow": "Other flow", "classification": {"classHierarchy": "Größen / Umweltliche Größen / EPD EN 15804 / LCI Indikatoren", "name": "GaBiCategories"}}, {"dataSetInternalID": 4, "referenceToFlowDataSet": {"shortDescription": [{"value": "Exported thermal energy (EET)", "lang": "en"}, {"value": "Exportierte thermische Energie (EET)", "lang": "de"}, {"value": "Energía exportada termal (EET)", "lang": "es"}], "type": "flow data set", "refObjectId": "98daf38a-7a79-46d3-9a37-2b7bd0955810", "version": "30.00.000"}, "exchange direction": "OUTPUT", "meanAmount": 0.0, "other": {"anies": [{"value": "0.0", "module": "A1", "scenario": "Standard Scenario"}, {"value": "0.0", "module": "A2", "scenario": "Standard Scenario"}, {"value": "-1.26", "module": "A3", "scenario": "Standard Scenario"}, {"value": "0.0", "module": "A4", "scenario": "Standard Scenario"}, {"value": "0.0", "module": "A5", "scenario": "Standard Scenario"}, {"value": "0.0", "module": "C1", "scenario": "Standard Scenario"}, {"value": "0.0", "module": "C2", "scenario": "Standard Scenario"}, {"value": "0.0", "module": "C3", "scenario": "Standard Scenario"}, {"value": "0.0", "module": "C4", "scenario": "Standard Scenario"}, {"value": "-43.1", "module": "D", "scenario": "Standard Scenario"}, {"name": "referenceToUnitGroupDataSet", "value": {"shortDescription": [{"value": "MJ"}], "type": "unit group data set", "refObjectId": "93a60a57-a3c8-11da-a746-0800200c9a66", "uri": "../unitgroups/93a60a57-a3c8-11da-a746-0800200c9a66"}}]}, "flowProperties": [], "typeOfFlow": "Other flow", "classification": {"classHierarchy": "Größen / Umweltliche Größen / EPD EN 15804 / LCI Indikatoren", "name": "GaBiCategories"}}, {"dataSetInternalID": 5, "referenceToFlowDataSet": {"shortDescription": [{"value": "Hazardous waste disposed (HWD)", "lang": "en"}, {"value": "Gefährlicher Abfall zur Deponie (HWD)", "lang": "de"}, {"value": "Residuos peligrosos eliminados (HWD)", "lang": "es"}], "type": "flow data set", "refObjectId": "430f9e0f-59b2-46a0-8e0d-55e0e84948fc", "version": "30.00.000"}, "exchange direction": "OUTPUT", "meanAmount": 0.0, "other": {"anies": [{"value": "1.07E-4", "module": "A1", "scenario": "Standard Scenario"}, {"value": "3.8E-5", "module": "A2", "scenario": "Standard Scenario"}, {"value": "1.86E-5", "module": "A3", "scenario": "Standard Scenario"}, {"value": "1.78E-5", "module": "A4", "scenario": "Standard Scenario"}, {"value": "5.23E-6", "module": "A5", "scenario": "Standard Scenario"}, {"value": "0.0", "module": "C1", "scenario": "Standard Scenario"}, {"value": "4.89E-6", "module": "C2", "scenario": "Standard Scenario"}, {"value": "3.65E-6", "module": "C3", "scenario": "Standard Scenario"}, {"value": "1.24E-7", "module": "C4", "scenario": "Standard Scenario"}, {"value": "-5.02E-5", "module": "D", "scenario": "Standard Scenario"}, {"name": "referenceToUnitGroupDataSet", "value": {"shortDescription": [{"value": "kg"}], "type": "unit group data set", "refObjectId": "ad38d542-3fe9-439d-9b95-2f5f7752acaf", "uri": "../unitgroups/ad38d542-3fe9-439d-9b95-2f5f7752acaf"}}]}, "flowProperties": [], "typeOfFlow": "Other flow", "classification": {"classHierarchy": "Größen / Umweltliche Größen / EPD EN 15804 / LCI Indikatoren", "name": "GaBiCategories"}}, {"dataSetInternalID": 6, "referenceToFlowDataSet": {"shortDescription": [{"value": "Materials for energy recovery (MER)", "lang": "en"}, {"value": "Stoffe für die Energierückgewinnung (MER)", "lang": "de"}, {"value": "Materiales para valorización energética (recuperación de energía) (MER)", "lang": "es"}], "type": "flow data set", "refObjectId": "59a9181c-3aaf-46ee-8b13-2b3723b6e447", "version": "30.00.000"}, "exchange direction": "OUTPUT", "meanAmount": 0.0, "other": {"anies": [{"value": "0.0", "module": "A1", "scenario": "Standard Scenario"}, {"value": "0.0", "module": "A2", "scenario": "Standard Scenario"}, {"value": "0.0", "module": "A3", "scenario": "Standard Scenario"}, {"value": "0.0", "module": "A4", "scenario": "Standard Scenario"}, {"value": "0.0", "module": "A5", "scenario": "Standard Scenario"}, {"value": "0.0", "module": "C1", "scenario": "Standard Scenario"}, {"value": "0.0", "module": "C2", "scenario": "Standard Scenario"}, {"value": "6.1", "module": "C3", "scenario": "Standard Scenario"}, {"value": "0.0", "module": "C4", "scenario": "Standard Scenario"}, {"value": "0.0", "module": "D", "scenario": "Standard Scenario"}, {"name": "referenceToUnitGroupDataSet", "value": {"shortDescription": [{"value": "kg"}], "type": "unit group data set", "refObjectId": "ad38d542-3fe9-439d-9b95-2f5f7752acaf", "uri": "../unitgroups/ad38d542-3fe9-439d-9b95-2f5f7752acaf"}}]}, "flowProperties": [], "typeOfFlow": "Other flow", "classification": {"classHierarchy": "Größen / Umweltliche Größen / EPD EN 15804 / LCI Indikatoren", "name": "GaBiCategories"}}, {"dataSetInternalID": 7, "referenceToFlowDataSet": {"shortDescription": [{"value": "Materials for recycling (MFR)", "lang": "en"}, {"value": "Stoffe zum Recycling (MFR)", "lang": "de"}, {"value": "Materiales para el reciclaje (MFR)", "lang": "es"}], "type": "flow data set", "refObjectId": "d7fe48a5-4103-49c8-9aae-b0b5dfdbd6ae", "version": "30.00.000"}, "exchange direction": "OUTPUT", "meanAmount": 0.0, "other": {"anies": [{"value": "0.0", "module": "A1", "scenario": "Standard Scenario"}, {"value": "0.0", "module": "A2", "scenario": "Standard Scenario"}, {"value": "0.0", "module": "A3", "scenario": "Standard Scenario"}, {"value": "0.0", "module": "A4", "scenario": "Standard Scenario"}, {"value": "1.78E-4", "module": "A5", "scenario": "Standard Scenario"}, {"value": "0.0", "module": "C1", "scenario": "Standard Scenario"}, {"value": "0.0", "module": "C2", "scenario": "Standard Scenario"}, {"value": "0.0", "module": "C3", "scenario": "Standard Scenario"}, {"value": "0.0", "module": "C4", "scenario": "Standard Scenario"}, {"value": "0.0", "module": "D", "scenario": "Standard Scenario"}, {"name": "referenceToUnitGroupDataSet", "value": {"shortDescription": [{"value": "kg"}], "type": "unit group data set", "refObjectId": "ad38d542-3fe9-439d-9b95-2f5f7752acaf", "uri": "../unitgroups/ad38d542-3fe9-439d-9b95-2f5f7752acaf"}}]}, "flowProperties": [], "typeOfFlow": "Other flow", "classification": {"classHierarchy": "Größen / Umweltliche Größen / EPD EN 15804 / LCI Indikatoren", "name": "GaBiCategories"}}, {"dataSetInternalID": 8, "referenceToFlowDataSet": {"shortDescription": [{"value": "Use of net fresh water (FW)", "lang": "en"}, {"value": "Einsatz von Süßwasserressourcen (FW)", "lang": "de"}, {"value": "Uso neto de recursos de agua dulce (FW)", "lang": "es"}], "type": "flow data set", "refObjectId": "3cf952c8-f3a4-461d-8c96-96456ca62246", "version": "30.00.000"}, "exchange direction": "INPUT", "meanAmount": 0.0, "other": {"anies": [{"value": "0.17", "module": "A1", "scenario": "Standard Scenario"}, {"value": "0.00183", "module": "A2", "scenario": "Standard Scenario"}, {"value": "0.00783", "module": "A3", "scenario": "Standard Scenario"}, {"value": "8.58E-4", "module": "A4", "scenario": "Standard Scenario"}, {"value": "0.00551", "module": "A5", "scenario": "Standard Scenario"}, {"value": "0.0", "module": "C1", "scenario": "Standard Scenario"}, {"value": "2.35E-4", "module": "C2", "scenario": "Standard Scenario"}, {"value": "0.00299", "module": "C3", "scenario": "Standard Scenario"}, {"value": "8.41E-5", "module": "C4", "scenario": "Standard Scenario"}, {"value": "-0.0163", "module": "D", "scenario": "Standard Scenario"}, {"name": "referenceToUnitGroupDataSet", "value": {"shortDescription": [{"value": "m3"}], "type": "unit group data set", "refObjectId": "cd950537-0a98-4044-9ba7-9f9a68d0a504", "uri": "../unitgroups/cd950537-0a98-4044-9ba7-9f9a68d0a504"}}]}, "flowProperties": [], "typeOfFlow": "Other flow", "classification": {"classHierarchy": "Größen / Umweltliche Größen / EPD EN 15804 / LCI Indikatoren", "name": "GaBiCategories"}}, {"dataSetInternalID": 9, "referenceToFlowDataSet": {"shortDescription": [{"value": "Non hazardous waste dispose (NHWD)", "lang": "en"}, {"value": "Entsorgter nicht gefährlicher Abfall (NHWD)", "lang": "de"}, {"value": "Residuos no peligrosos eliminados (NHWD)", "lang": "es"}], "type": "flow data set", "refObjectId": "b29ef66b-e286-4afa-949f-62f1a7b4d7fa", "version": "30.00.000"}, "exchange direction": "OUTPUT", "meanAmount": 0.0, "other": {"anies": [{"value": "0.872", "module": "A1", "scenario": "Standard Scenario"}, {"value": "0.951", "module": "A2", "scenario": "Standard Scenario"}, {"value": "0.0872", "module": "A3", "scenario": "Standard Scenario"}, {"value": "0.447", "module": "A4", "scenario": "Standard Scenario"}, {"value": "0.0728", "module": "A5", "scenario": "Standard Scenario"}, {"value": "0.0", "module": "C1", "scenario": "Standard Scenario"}, {"value": "0.122", "module": "C2", "scenario": "Standard Scenario"}, {"value": "0.321", "module": "C3", "scenario": "Standard Scenario"}, {"value": "0.322", "module": "C4", "scenario": "Standard Scenario"}, {"value": "-0.158", "module": "D", "scenario": "Standard Scenario"}, {"name": "referenceToUnitGroupDataSet", "value": {"shortDescription": [{"value": "kg"}], "type": "unit group data set", "refObjectId": "ad38d542-3fe9-439d-9b95-2f5f7752acaf", "uri": "../unitgroups/ad38d542-3fe9-439d-9b95-2f5f7752acaf"}}]}, "flowProperties": [], "typeOfFlow": "Other flow", "classification": {"classHierarchy": "Größen / Umweltliche Größen / EPD EN 15804 / LCI Indikatoren", "name": "GaBiCategories"}}, {"dataSetInternalID": 10, "referenceToFlowDataSet": {"shortDescription": [{"value": "Use of non renewable primary energy (PENRE)", "lang": "en"}, {"value": "Nicht-erneuerbare Primärenergie als Energieträger (PENRE)", "lang": "de"}, {"value": "Uso de energía primaria no renovable, excluyendo los recursos de energía primaria no renovable utilizada como materia prima (PENRE)", "lang": "es"}], "type": "flow data set", "refObjectId": "ac857178-2b45-46ec-892a-a9a4332f0372", "version": "30.00.000"}, "exchange direction": "INPUT", "meanAmount": 0.0, "other": {"anies": [{"value": "110.0", "module": "A1", "scenario": "Standard Scenario"}, {"value": "15.9", "module": "A2", "scenario": "Standard Scenario"}, {"value": "16.4", "module": "A3", "scenario": "Standard Scenario"}, {"value": "7.48", "module": "A4", "scenario": "Standard Scenario"}, {"value": "4.41", "module": "A5", "scenario": "Standard Scenario"}, {"value": "0.0", "module": "C1", "scenario": "Standard Scenario"}, {"value": "2.05", "module": "C2", "scenario": "Standard Scenario"}, {"value": "0.872", "module": "C3", "scenario": "Standard Scenario"}, {"value": "0.0869", "module": "C4", "scenario": "Standard Scenario"}, {"value": "-74.5", "module": "D", "scenario": "Standard Scenario"}, {"name": "referenceToUnitGroupDataSet", "value": {"shortDescription": [{"value": "MJ"}], "type": "unit group data set", "refObjectId": "93a60a57-a3c8-11da-a746-0800200c9a66", "uri": "../unitgroups/93a60a57-a3c8-11da-a746-0800200c9a66"}}]}, "flowProperties": [], "typeOfFlow": "Other flow", "classification": {"classHierarchy": "Größen / Umweltliche Größen / EPD EN 15804 / LCI Indikatoren", "name": "GaBiCategories"}}, {"dataSetInternalID": 11, "referenceToFlowDataSet": {"shortDescription": [{"value": "Use of non renewable primary energy resources used as raw materials (PENRM)", "lang": "en"}, {"value": "Nicht-erneuerbare Primärenergie zur stofflichen Nutzung (PENRM)", "lang": "de"}, {"value": "Uso de la energía primaria no renovable utilizada como materia prima (PENRM)", "lang": "es"}], "type": "flow data set", "refObjectId": "1421caa0-679d-4bf4-b282-0eb850ccae27", "version": "30.00.000"}, "exchange direction": "INPUT", "meanAmount": 0.0, "other": {"anies": [{"value": "6.13", "module": "A1", "scenario": "Standard Scenario"}, {"value": "0.0", "module": "A2", "scenario": "Standard Scenario"}, {"value": "0.234", "module": "A3", "scenario": "Standard Scenario"}, {"value": "0.0", "module": "A4", "scenario": "Standard Scenario"}, {"value": "0.191", "module": "A5", "scenario": "Standard Scenario"}, {"value": "0.0", "module": "C1", "scenario": "Standard Scenario"}, {"value": "0.0", "module": "C2", "scenario": "Standard Scenario"}, {"value": "0.0", "module": "C3", "scenario": "Standard Scenario"}, {"value": "0.0", "module": "C4", "scenario": "Standard Scenario"}, {"value": "-6.78E-5", "module": "D", "scenario": "Standard Scenario"}, {"name": "referenceToUnitGroupDataSet", "value": {"shortDescription": [{"value": "MJ"}], "type": "unit group data set", "refObjectId": "93a60a57-a3c8-11da-a746-0800200c9a66", "uri": "../unitgroups/93a60a57-a3c8-11da-a746-0800200c9a66"}}]}, "flowProperties": [], "typeOfFlow": "Other flow", "classification": {"classHierarchy": "Größen / Umweltliche Größen / EPD EN 15804 / LCI Indikatoren", "name": "GaBiCategories"}}, {"dataSetInternalID": 12, "referenceToFlowDataSet": {"shortDescription": [{"value": "Use of non renewable secondary fuels (NRSF)", "lang": "en"}, {"value": "Nicht erneuerbare Sekundärbrennstoffe (NRSF)", "lang": "de"}, {"value": "Uso de combustibles secundarios no renovables (NRSF)", "lang": "es"}], "type": "flow data set", "refObjectId": "89def144-d39a-4287-b86f-efde453ddcb2", "version": "30.00.000"}, "exchange direction": "INPUT", "meanAmount": 0.0, "other": {"anies": [{"value": "0.0", "module": "A1", "scenario": "Standard Scenario"}, {"value": "0.0", "module": "A2", "scenario": "Standard Scenario"}, {"value": "0.0", "module": "A3", "scenario": "Standard Scenario"}, {"value": "0.0", "module": "A4", "scenario": "Standard Scenario"}, {"value": "0.0", "module": "A5", "scenario": "Standard Scenario"}, {"value": "0.0", "module": "C1", "scenario": "Standard Scenario"}, {"value": "0.0", "module": "C2", "scenario": "Standard Scenario"}, {"value": "0.0", "module": "C3", "scenario": "Standard Scenario"}, {"value": "0.0", "module": "C4", "scenario": "Standard Scenario"}, {"value": "0.0", "module": "D", "scenario": "Standard Scenario"}, {"name": "referenceToUnitGroupDataSet", "value": {"shortDescription": [{"value": "MJ"}], "type": "unit group data set", "refObjectId": "93a60a57-a3c8-11da-a746-0800200c9a66", "uri": "../unitgroups/93a60a57-a3c8-11da-a746-0800200c9a66"}}]}, "flowProperties": [], "typeOfFlow": "Other flow", "classification": {"classHierarchy": "Größen / Umweltliche Größen / EPD EN 15804 / LCI Indikatoren", "name": "GaBiCategories"}}, {"dataSetInternalID": 13, "referenceToFlowDataSet": {"shortDescription": [{"value": "Radioactive waste disposed (RWD)", "lang": "en"}, {"value": "Entsorgter radioaktiver Abfall (RWD)", "lang": "de"}, {"value": "Residuos radiactivos eliminados (RWD)", "lang": "es"}], "type": "flow data set", "refObjectId": "3449546e-52ad-4b39-b809-9fb77cea8ff6", "version": "30.00.000"}, "exchange direction": "OUTPUT", "meanAmount": 0.0, "other": {"anies": [{"value": "3.03E-4", "module": "A1", "scenario": "Standard Scenario"}, {"value": "9.85E-5", "module": "A2", "scenario": "Standard Scenario"}, {"value": "2.32E-5", "module": "A3", "scenario": "Standard Scenario"}, {"value": "4.62E-5", "module": "A4", "scenario": "Standard Scenario"}, {"value": "1.34E-5", "module": "A5", "scenario": "Standard Scenario"}, {"value": "0.0", "module": "C1", "scenario": "Standard Scenario"}, {"value": "1.27E-5", "module": "C2", "scenario": "Standard Scenario"}, {"value": "1.75E-6", "module": "C3", "scenario": "Standard Scenario"}, {"value": "4.79E-7", "module": "C4", "scenario": "Standard Scenario"}, {"value": "-1.72E-4", "module": "D", "scenario": "Standard Scenario"}, {"name": "referenceToUnitGroupDataSet", "value": {"shortDescription": [{"value": "kg"}], "type": "unit group data set", "refObjectId": "ad38d542-3fe9-439d-9b95-2f5f7752acaf", "uri": "../unitgroups/ad38d542-3fe9-439d-9b95-2f5f7752acaf"}}]}, "flowProperties": [], "typeOfFlow": "Other flow", "classification": {"classHierarchy": "Größen / Umweltliche Größen / EPD EN 15804 / LCI Indikatoren", "name": "GaBiCategories"}}, {"dataSetInternalID": 14, "referenceToFlowDataSet": {"shortDescription": [{"value": "Use of renewable primary energy (PERE)", "lang": "en"}, {"value": "Erneuerbare Primärenergie als Energieträger (PERE)", "lang": "de"}, {"value": "Uso de energía primaria renovable excluyendo los recursos de energía primaria renovable utilizada como materia prima (PERE)", "lang": "es"}], "type": "flow data set", "refObjectId": "20f32be5-0398-4288-9b6d-accddd195317", "version": "30.00.000"}, "exchange direction": "INPUT", "meanAmount": 0.0, "other": {"anies": [{"value": "-6.49", "module": "A1", "scenario": "Standard Scenario"}, {"value": "0.188", "module": "A2", "scenario": "Standard Scenario"}, {"value": "2.18", "module": "A3", "scenario": "Standard Scenario"}, {"value": "0.0881", "module": "A4", "scenario": "Standard Scenario"}, {"value": "-0.118", "module": "A5", "scenario": "Standard Scenario"}, {"value": "0.0", "module": "C1", "scenario": "Standard Scenario"}, {"value": "0.0242", "module": "C2", "scenario": "Standard Scenario"}, {"value": "0.0265", "module": "C3", "scenario": "Standard Scenario"}, {"value": "0.00172", "module": "C4", "scenario": "Standard Scenario"}, {"value": "-4.78", "module": "D", "scenario": "Standard Scenario"}, {"name": "referenceToUnitGroupDataSet", "value": {"shortDescription": [{"value": "MJ"}], "type": "unit group data set", "refObjectId": "93a60a57-a3c8-11da-a746-0800200c9a66", "uri": "../unitgroups/93a60a57-a3c8-11da-a746-0800200c9a66"}}]}, "flowProperties": [], "typeOfFlow": "Other flow", "classification": {"classHierarchy": "Größen / Umweltliche Größen / EPD EN 15804 / LCI Indikatoren", "name": "GaBiCategories"}}, {"dataSetInternalID": 15, "referenceToFlowDataSet": {"shortDescription": [{"value": "Use of renewable primary energy resources used as raw materials (PERM)", "lang": "en"}, {"value": "Erneuerbare Primärenergie zur stofflichen Nutzung (PERM)", "lang": "de"}, {"value": "Uso de energía primaria renovable utilizada como materia prima (PERM)", "lang": "es"}], "type": "flow data set", "refObjectId": "fb3ec0de-548d-4508-aea5-00b73bf6f702", "version": "30.00.000"}, "exchange direction": "INPUT", "meanAmount": 0.0, "other": {"anies": [{"value": "83.8", "module": "A1", "scenario": "Standard Scenario"}, {"value": "0.0", "module": "A2", "scenario": "Standard Scenario"}, {"value": "2.51", "module": "A3", "scenario": "Standard Scenario"}, {"value": "0.0", "module": "A4", "scenario": "Standard Scenario"}, {"value": "2.59", "module": "A5", "scenario": "Standard Scenario"}, {"value": "0.0", "module": "C1", "scenario": "Standard Scenario"}, {"value": "0.0", "module": "C2", "scenario": "Standard Scenario"}, {"value": "0.0", "module": "C3", "scenario": "Standard Scenario"}, {"value": "0.0", "module": "C4", "scenario": "Standard Scenario"}, {"value": "-0.00245", "module": "D", "scenario": "Standard Scenario"}, {"name": "referenceToUnitGroupDataSet", "value": {"shortDescription": [{"value": "MJ"}], "type": "unit group data set", "refObjectId": "93a60a57-a3c8-11da-a746-0800200c9a66", "uri": "../unitgroups/93a60a57-a3c8-11da-a746-0800200c9a66"}}]}, "flowProperties": [], "typeOfFlow": "Other flow", "classification": {"classHierarchy": "Größen / Umweltliche Größen / EPD EN 15804 / LCI Indikatoren", "name": "GaBiCategories"}}, {"dataSetInternalID": 16, "referenceToFlowDataSet": {"shortDescription": [{"value": "Use of renewable secondary fuels (RSF)", "lang": "en"}, {"value": "Erneuerbare Sekundärbrennstoffe (RSF)", "lang": "de"}, {"value": "Uso de combustibles secundarios renovables (RSF)", "lang": "es"}], "type": "flow data set", "refObjectId": "64333088-a55f-4aa2-9a31-c10b07816787", "version": "30.00.000"}, "exchange direction": "INPUT", "meanAmount": 0.0, "other": {"anies": [{"value": "0.0", "module": "A1", "scenario": "Standard Scenario"}, {"value": "0.0", "module": "A2", "scenario": "Standard Scenario"}, {"value": "0.0", "module": "A3", "scenario": "Standard Scenario"}, {"value": "0.0", "module": "A4", "scenario": "Standard Scenario"}, {"value": "0.0", "module": "A5", "scenario": "Standard Scenario"}, {"value": "0.0", "module": "C1", "scenario": "Standard Scenario"}, {"value": "0.0", "module": "C2", "scenario": "Standard Scenario"}, {"value": "0.0", "module": "C3", "scenario": "Standard Scenario"}, {"value": "0.0", "module": "C4", "scenario": "Standard Scenario"}, {"value": "0.0", "module": "D", "scenario": "Standard Scenario"}, {"name": "referenceToUnitGroupDataSet", "value": {"shortDescription": [{"value": "MJ"}], "type": "unit group data set", "refObjectId": "93a60a57-a3c8-11da-a746-0800200c9a66", "uri": "../unitgroups/93a60a57-a3c8-11da-a746-0800200c9a66"}}]}, "flowProperties": [], "typeOfFlow": "Other flow", "classification": {"classHierarchy": "Größen / Umweltliche Größen / EPD EN 15804 / LCI Indikatoren", "name": "GaBiCategories"}}, {"dataSetInternalID": 17, "referenceToFlowDataSet": {"shortDescription": [{"value": "Use of secondary material (SM)", "lang": "en"}, {"value": "Einsatz von Sekundärstoffen (SM)", "lang": "de"}, {"value": "Uso de materiales secundarios (SM)", "lang": "es"}], "type": "flow data set", "refObjectId": "c6a1f35f-2d09-4f54-8dfb-97e502e1ce92", "version": "30.00.000"}, "exchange direction": "INPUT", "meanAmount": 0.0, "other": {"anies": [{"value": "0.0", "module": "A1", "scenario": "Standard Scenario"}, {"value": "0.0", "module": "A2", "scenario": "Standard Scenario"}, {"value": "0.0", "module": "A3", "scenario": "Standard Scenario"}, {"value": "0.0", "module": "A4", "scenario": "Standard Scenario"}, {"value": "0.0", "module": "A5", "scenario": "Standard Scenario"}, {"value": "0.0", "module": "C1", "scenario": "Standard Scenario"}, {"value": "0.0", "module": "C2", "scenario": "Standard Scenario"}, {"value": "0.0", "module": "C3", "scenario": "Standard Scenario"}, {"value": "0.0", "module": "C4", "scenario": "Standard Scenario"}, {"value": "0.0", "module": "D", "scenario": "Standard Scenario"}, {"name": "referenceToUnitGroupDataSet", "value": {"shortDescription": [{"value": "kg"}], "type": "unit group data set", "refObjectId": "ad38d542-3fe9-439d-9b95-2f5f7752acaf", "uri": "../unitgroups/ad38d542-3fe9-439d-9b95-2f5f7752acaf"}}]}, "flowProperties": [], "typeOfFlow": "Other flow", "classification": {"classHierarchy": "Größen / Umweltliche Größen / EPD EN 15804 / LCI Indikatoren", "name": "GaBiCategories"}}, {"dataSetInternalID": 18, "referenceToFlowDataSet": {"shortDescription": [{"value": "Total use of non renewable primary energy resource (PENRT)", "lang": "en"}, {"value": "Total nicht erneuerbare Primärenergie (PENRT)", "lang": "de"}, {"value": "Uso total de la energía primaria no renovable (energía primaria y recursos de energía primaria renovable utilizada como materia prima) (PENRT)", "lang": "es"}], "type": "flow data set", "refObjectId": "06159210-646b-4c8d-8583-da9b3b95a6c1", "version": "30.00.000"}, "exchange direction": "INPUT", "meanAmount": 0.0, "other": {"anies": [{"value": "116.0", "module": "A1", "scenario": "Standard Scenario"}, {"value": "15.9", "module": "A2", "scenario": "Standard Scenario"}, {"value": "16.6", "module": "A3", "scenario": "Standard Scenario"}, {"value": "7.48", "module": "A4", "scenario": "Standard Scenario"}, {"value": "4.6", "module": "A5", "scenario": "Standard Scenario"}, {"value": "0.0", "module": "C1", "scenario": "Standard Scenario"}, {"value": "2.05", "module": "C2", "scenario": "Standard Scenario"}, {"value": "0.614", "module": "C3", "scenario": "Standard Scenario"}, {"value": "0.0856", "module": "C4", "scenario": "Standard Scenario"}, {"value": "-74.5", "module": "D", "scenario": "Standard Scenario"}, {"name": "referenceToUnitGroupDataSet", "value": {"shortDescription": [{"value": "MJ"}], "type": "unit group data set", "refObjectId": "93a60a57-a3c8-11da-a746-0800200c9a66", "uri": "../unitgroups/93a60a57-a3c8-11da-a746-0800200c9a66"}}]}, "flowProperties": [], "typeOfFlow": "Other flow", "classification": {"classHierarchy": "Größen / Umweltliche Größen / EPD EN 15804 / LCI Indikatoren", "name": "GaBiCategories"}}, {"dataSetInternalID": 19, "referenceToFlowDataSet": {"shortDescription": [{"value": "Total use of renewable primary energy resources (PERT)", "lang": "en"}, {"value": "Total erneuerbare Primärenergie (PERT)", "lang": "de"}, {"value": "Uso total de la energía primaria renovable (energía primaria y recursos de energía primaria renovable utilizada como materia prima) (PERT)", "lang": "es"}], "type": "flow data set", "refObjectId": "53f97275-fa8a-4cdd-9024-65936002acd0", "version": "30.00.000"}, "exchange direction": "INPUT", "meanAmount": 0.0, "other": {"anies": [{"value": "77.3", "module": "A1", "scenario": "Standard Scenario"}, {"value": "0.188", "module": "A2", "scenario": "Standard Scenario"}, {"value": "4.69", "module": "A3", "scenario": "Standard Scenario"}, {"value": "0.0881", "module": "A4", "scenario": "Standard Scenario"}, {"value": "2.47", "module": "A5", "scenario": "Standard Scenario"}, {"value": "0.0", "module": "C1", "scenario": "Standard Scenario"}, {"value": "0.0242", "module": "C2", "scenario": "Standard Scenario"}, {"value": "0.0263", "module": "C3", "scenario": "Standard Scenario"}, {"value": "0.00142", "module": "C4", "scenario": "Standard Scenario"}, {"value": "-4.79", "module": "D", "scenario": "Standard Scenario"}, {"name": "referenceToUnitGroupDataSet", "value": {"shortDescription": [{"value": "MJ"}], "type": "unit group data set", "refObjectId": "93a60a57-a3c8-11da-a746-0800200c9a66", "uri": "../unitgroups/93a60a57-a3c8-11da-a746-0800200c9a66"}}]}, "flowProperties": [], "typeOfFlow": "Other flow", "classification": {"classHierarchy": "Größen / Umweltliche Größen / EPD EN 15804 / LCI Indikatoren", "name": "GaBiCategories"}}]}, "LCIAResults": {"LCIAResult": [{"referenceToLCIAMethodDataSet": {"shortDescription": [{"value": "Abiotic depletion potential - non-fossil resources (ADPE)", "lang": "en"}, {"value": "Potenzial für die Verknappung abiotischer Ressourcen – nicht fossile Ressourcen (ADPE)", "lang": "de"}], "type": "LCIA method data set", "refObjectId": "b2ad6494-c78d-11e6-9d9d-cec0c932ce01", "version": "01.00.011"}, "meanAmount": 0.0, "other": {"anies": [{"value": "1.07E-4", "module": "A1", "scenario": "Standard Scenario"}, {"value": "2.52E-5", "module": "A2", "scenario": "Standard Scenario"}, {"value": "5.72E-6", "module": "A3", "scenario": "Standard Scenario"}, {"value": "1.18E-5", "module": "A4", "scenario": "Standard Scenario"}, {"value": "4.26E-6", "module": "A5", "scenario": "Standard Scenario"}, {"value": "0.0", "module": "C1", "scenario": "Standard Scenario"}, {"value": "3.24E-6", "module": "C2", "scenario": "Standard Scenario"}, {"value": "3.51E-7", "module": "C3", "scenario": "Standard Scenario"}, {"value": "3.65E-8", "module": "C4", "scenario": "Standard Scenario"}, {"value": "-8.63E-6", "module": "D", "scenario": "Standard Scenario"}, {"name": "referenceToUnitGroupDataSet", "value": {"shortDescription": [{"value": "kg Sb-Äqv."}], "type": "unit group data set", "refObjectId": "54ccd2d9-a32a-4fc2-923d-f2c8c93e89d4", "uri": "../unitgroups/54ccd2d9-a32a-4fc2-923d-f2c8c93e89d4"}}]}}, {"referenceToLCIAMethodDataSet": {"shortDescription": [{"value": "Abiotic depletion potential - fossil resources (ADPF)", "lang": "en"}, {"value": "Potenzial für die Verknappung abiotischer Ressourcen – fossile Brennstoffe (ADPF)", "lang": "de"}], "type": "LCIA method data set", "refObjectId": "b2ad6110-c78d-11e6-9d9d-cec0c932ce01", "version": "01.00.011"}, "meanAmount": 0.0, "other": {"anies": [{"value": "107.0", "module": "A1", "scenario": "Standard Scenario"}, {"value": "15.0", "module": "A2", "scenario": "Standard Scenario"}, {"value": "15.2", "module": "A3", "scenario": "Standard Scenario"}, {"value": "7.04", "module": "A4", "scenario": "Standard Scenario"}, {"value": "4.26", "module": "A5", "scenario": "Standard Scenario"}, {"value": "0.0", "module": "C1", "scenario": "Standard Scenario"}, {"value": "1.93", "module": "C2", "scenario": "Standard Scenario"}, {"value": "0.57", "module": "C3", "scenario": "Standard Scenario"}, {"value": "0.0806", "module": "C4", "scenario": "Standard Scenario"}, {"value": "-68.4", "module": "D", "scenario": "Standard Scenario"}, {"name": "referenceToUnitGroupDataSet", "value": {"shortDescription": [{"value": "MJ"}], "type": "unit group data set", "refObjectId": "93a60a57-a3c8-11da-a746-0800200c9a66", "uri": "../unitgroups/93a60a57-a3c8-11da-a746-0800200c9a66"}}]}}, {"referenceToLCIAMethodDataSet": {"shortDescription": [{"value": "Acidification potential, Accumulated Exceedance (AP)", "lang": "en"}, {"value": "Versauerungspotenzial, kumulierte Überschreitung (AP)", "lang": "de"}], "type": "LCIA method data set", "refObjectId": "b5c611c6-def3-11e6-bf01-fe55135034f3", "version": "01.03.011", "uri": "http://lca.jrc.ec.europa.eu/lcainfohub/datasets/elcd/lciamethods/f6cbd466-253f-4145-a4bb-8dae7d266e89.xml"}, "meanAmount": 0.0, "other": {"anies": [{"value": "0.0408", "module": "A1", "scenario": "Standard Scenario"}, {"value": "0.00577", "module": "A2", "scenario": "Standard Scenario"}, {"value": "0.00259", "module": "A3", "scenario": "Standard Scenario"}, {"value": "0.00271", "module": "A4", "scenario": "Standard Scenario"}, {"value": "0.00156", "module": "A5", "scenario": "Standard Scenario"}, {"value": "0.0", "module": "C1", "scenario": "Standard Scenario"}, {"value": "7.42E-4", "module": "C2", "scenario": "Standard Scenario"}, {"value": "0.00192", "module": "C3", "scenario": "Standard Scenario"}, {"value": "2.95E-5", "module": "C4", "scenario": "Standard Scenario"}, {"value": "-0.00877", "module": "D", "scenario": "Standard Scenario"}, {"name": "referenceToUnitGroupDataSet", "value": {"shortDescription": [{"value": "mol H+ eqv."}], "type": "unit group data set", "refObjectId": "42e089ac-92bf-4bf2-8ca1-5fc40d18f2ed", "uri": "../unitgroups/42e089ac-92bf-4bf2-8ca1-5fc40d18f2ed"}}]}}, {"referenceToLCIAMethodDataSet": {"shortDescription": [{"value": "Eutrophication potential - freshwater (EP-freshwater)", "lang": "en"}, {"value": "Eutrophierungspotenzial - Süßwasser (EP-freshwater)", "lang": "de"}], "type": "LCIA method data set", "refObjectId": "b53ec18f-7377-4ad3-86eb-cc3f4f276b2b", "version": "01.00.011", "uri": "http://lca.jrc.ec.europa.eu/lcainfohub/datasets/elcd/lciamethods/a4630d5b-df2f-48ae-b3f2-5e5257606d68.xml"}, "meanAmount": 0.0, "other": {"anies": [{"value": "2.93E-4", "module": "A1", "scenario": "Standard Scenario"}, {"value": "1.0E-5", "module": "A2", "scenario": "Standard Scenario"}, {"value": "1.76E-5", "module": "A3", "scenario": "Standard Scenario"}, {"value": "4.71E-6", "module": "A4", "scenario": "Standard Scenario"}, {"value": "1.01E-5", "module": "A5", "scenario": "Standard Scenario"}, {"value": "0.0", "module": "C1", "scenario": "Standard Scenario"}, {"value": "1.29E-6", "module": "C2", "scenario": "Standard Scenario"}, {"value": "1.15E-6", "module": "C3", "scenario": "Standard Scenario"}, {"value": "7.1E-8", "module": "C4", "scenario": "Standard Scenario"}, {"value": "-4.22E-4", "module": "D", "scenario": "Standard Scenario"}, {"name": "referenceToUnitGroupDataSet", "value": {"shortDescription": [{"value": "kg P eqv."}], "type": "unit group data set", "refObjectId": "0429039d-a61d-4590-ba67-aa4a20a810a1", "uri": "../unitgroups/0429039d-a61d-4590-ba67-aa4a20a810a1"}}]}}, {"referenceToLCIAMethodDataSet": {"shortDescription": [{"value": "Eutrophication potential - marine (EP-marine)", "lang": "en"}, {"value": "Eutrophierungspotenzial - Salzwasser (EP-marine)", "lang": "de"}], "type": "LCIA method data set", "refObjectId": "b5c619fa-def3-11e6-bf01-fe55135034f3", "version": "02.00.011", "uri": "http://lca.jrc.ec.europa.eu/lcainfohub/datasets/elcd/lciamethods/5296e2be-060b-4e50-b033-d45f85f6ac92.xml"}, "meanAmount": 0.0, "other": {"anies": [{"value": "0.00753", "module": "A1", "scenario": "Standard Scenario"}, {"value": "0.00203", "module": "A2", "scenario": "Standard Scenario"}, {"value": "6.03E-4", "module": "A3", "scenario": "Standard Scenario"}, {"value": "9.54E-4", "module": "A4", "scenario": "Standard Scenario"}, {"value": "3.42E-4", "module": "A5", "scenario": "Standard Scenario"}, {"value": "0.0", "module": "C1", "scenario": "Standard Scenario"}, {"value": "2.61E-4", "module": "C2", "scenario": "Standard Scenario"}, {"value": "8.89E-4", "module": "C3", "scenario": "Standard Scenario"}, {"value": "1.91E-5", "module": "C4", "scenario": "Standard Scenario"}, {"value": "-0.00161", "module": "D", "scenario": "Standard Scenario"}, {"name": "referenceToUnitGroupDataSet", "value": {"shortDescription": [{"value": "kg N eqv."}], "type": "unit group data set", "refObjectId": "d05bb823-ecdf-4686-8c40-bf1d9257859f", "uri": "../unitgroups/d05bb823-ecdf-4686-8c40-bf1d9257859f"}}]}}, {"referenceToLCIAMethodDataSet": {"shortDescription": [{"value": "Eutrophication potential - terrestrial (EP-terrestrial)", "lang": "en"}, {"value": "Eutrophierungspotenzial - Land (EP-terrestrial)", "lang": "de"}], "type": "LCIA method data set", "refObjectId": "b5c614d2-def3-11e6-bf01-fe55135034f3", "version": "01.02.010", "uri": "http://lca.jrc.ec.europa.eu/lcainfohub/datasets/elcd/lciamethods/40054970-5936-477c-9bec-29fa23b1cb77.xml"}, "meanAmount": 0.0, "other": {"anies": [{"value": "0.108", "module": "A1", "scenario": "Standard Scenario"}, {"value": "0.0224", "module": "A2", "scenario": "Standard Scenario"}, {"value": "0.00743", "module": "A3", "scenario": "Standard Scenario"}, {"value": "0.0105", "module": "A4", "scenario": "Standard Scenario"}, {"value": "0.00455", "module": "A5", "scenario": "Standard Scenario"}, {"value": "0.0", "module": "C1", "scenario": "Standard Scenario"}, {"value": "0.00288", "module": "C2", "scenario": "Standard Scenario"}, {"value": "0.0102", "module": "C3", "scenario": "Standard Scenario"}, {"value": "1.09E-4", "module": "C4", "scenario": "Standard Scenario"}, {"value": "-0.0238", "module": "D", "scenario": "Standard Scenario"}, {"name": "referenceToUnitGroupDataSet", "value": {"shortDescription": [{"value": "mol N eqv."}], "type": "unit group data set", "refObjectId": "71b4d617-0ec9-4d3f-b65e-e438940c2401", "uri": "../unitgroups/71b4d617-0ec9-4d3f-b65e-e438940c2401"}}]}}, {"referenceToLCIAMethodDataSet": {"shortDescription": [{"value": "Global Warming Potential - total (GWP-total)", "lang": "en"}, {"value": "Globales Erwärmungspotenzial - total (GWP-total)", "lang": "de"}], "type": "LCIA method data set", "refObjectId": "6a37f984-a4b3-458a-a20a-64418c145fa2", "version": "04.00.017"}, "meanAmount": 0.0, "other": {"anies": [{"value": "2.06", "module": "A1", "scenario": "Standard Scenario"}, {"value": "0.995", "module": "A2", "scenario": "Standard Scenario"}, {"value": "0.956", "module": "A3", "scenario": "Standard Scenario"}, {"value": "0.467", "module": "A4", "scenario": "Standard Scenario"}, {"value": "0.402", "module": "A5", "scenario": "Standard Scenario"}, {"value": "0.0", "module": "C1", "scenario": "Standard Scenario"}, {"value": "0.128", "module": "C2", "scenario": "Standard Scenario"}, {"value": "8.91", "module": "C3", "scenario": "Standard Scenario"}, {"value": "0.0358", "module": "C4", "scenario": "Standard Scenario"}, {"value": "-4.89", "module": "D", "scenario": "Standard Scenario"}, {"name": "referenceToUnitGroupDataSet", "value": {"shortDescription": [{"value": "kg CO2-Äqv."}], "type": "unit group data set", "refObjectId": "1ebf3012-d0db-4de2-aefd-ef30cedb0be1", "uri": "../unitgroups/1ebf3012-d0db-4de2-aefd-ef30cedb0be1"}}]}}, {"referenceToLCIAMethodDataSet": {"shortDescription": [{"value": "Global Warming Potential - fossil fuels (GWP-fossil)", "lang": "en"}, {"value": "Globales Erwärmungspotenzial - fossil (GWP-fossil)", "lang": "de"}], "type": "LCIA method data set", "refObjectId": "5f635281-343e-44fb-83df-1971b155e6b6", "version": "01.00.009"}, "meanAmount": 0.0, "other": {"anies": [{"value": "6.05", "module": "A1", "scenario": "Standard Scenario"}, {"value": "0.994", "module": "A2", "scenario": "Standard Scenario"}, {"value": "0.978", "module": "A3", "scenario": "Standard Scenario"}, {"value": "0.467", "module": "A4", "scenario": "Standard Scenario"}, {"value": "0.251", "module": "A5", "scenario": "Standard Scenario"}, {"value": "0.0", "module": "C1", "scenario": "Standard Scenario"}, {"value": "0.128", "module": "C2", "scenario": "Standard Scenario"}, {"value": "0.056", "module": "C3", "scenario": "Standard Scenario"}, {"value": "0.00382", "module": "C4", "scenario": "Standard Scenario"}, {"value": "-4.66", "module": "D", "scenario": "Standard Scenario"}, {"name": "referenceToUnitGroupDataSet", "value": {"shortDescription": [{"value": "kg CO2-Äqv."}], "type": "unit group data set", "refObjectId": "1ebf3012-d0db-4de2-aefd-ef30cedb0be1", "uri": "../unitgroups/1ebf3012-d0db-4de2-aefd-ef30cedb0be1"}}]}}, {"referenceToLCIAMethodDataSet": {"shortDescription": [{"value": "Global Warming Potential - biogenic (GWP-biogenic)", "lang": "en"}, {"value": "Globales Erwärmungspotenzial - biogen (GWP-biogenic)", "lang": "de"}], "type": "LCIA method data set", "refObjectId": "2356e1ab-0185-4db5-86e5-16de51c7485c", "version": "01.00.006"}, "meanAmount": 0.0, "other": {"anies": [{"value": "-3.99", "module": "A1", "scenario": "Standard Scenario"}, {"value": "4.59E-4", "module": "A2", "scenario": "Standard Scenario"}, {"value": "-0.0225", "module": "A3", "scenario": "Standard Scenario"}, {"value": "2.16E-4", "module": "A4", "scenario": "Standard Scenario"}, {"value": "0.151", "module": "A5", "scenario": "Standard Scenario"}, {"value": "0.0", "module": "C1", "scenario": "Standard Scenario"}, {"value": "5.91E-5", "module": "C2", "scenario": "Standard Scenario"}, {"value": "8.86", "module": "C3", "scenario": "Standard Scenario"}, {"value": "0.032", "module": "C4", "scenario": "Standard Scenario"}, {"value": "-0.228", "module": "D", "scenario": "Standard Scenario"}, {"name": "referenceToUnitGroupDataSet", "value": {"shortDescription": [{"value": "kg CO2-Äqv."}], "type": "unit group data set", "refObjectId": "1ebf3012-d0db-4de2-aefd-ef30cedb0be1", "uri": "../unitgroups/1ebf3012-d0db-4de2-aefd-ef30cedb0be1"}}]}}, {"referenceToLCIAMethodDataSet": {"shortDescription": [{"value": "Global Warming Potential - land use and land use change (GWP-luluc)", "lang": "en"}, {"value": "Globales Erwärmungspotenzial - luluc (GWP-luluc)", "lang": "de"}], "type": "LCIA method data set", "refObjectId": "4331bbdb-978a-490d-8707-eeb047f01a55", "version": "01.00.006"}, "meanAmount": 0.0, "other": {"anies": [{"value": "0.00752", "module": "A1", "scenario": "Standard Scenario"}, {"value": "3.64E-4", "module": "A2", "scenario": "Standard Scenario"}, {"value": "3.46E-4", "module": "A3", "scenario": "Standard Scenario"}, {"value": "1.71E-4", "module": "A4", "scenario": "Standard Scenario"}, {"value": "2.52E-4", "module": "A5", "scenario": "Standard Scenario"}, {"value": "0.0", "module": "C1", "scenario": "Standard Scenario"}, {"value": "4.69E-5", "module": "C2", "scenario": "Standard Scenario"}, {"value": "1.53E-5", "module": "C3", "scenario": "Standard Scenario"}, {"value": "1.67E-6", "module": "C4", "scenario": "Standard Scenario"}, {"value": "-0.00338", "module": "D", "scenario": "Standard Scenario"}, {"name": "referenceToUnitGroupDataSet", "value": {"shortDescription": [{"value": "kg CO2-Äqv."}], "type": "unit group data set", "refObjectId": "1ebf3012-d0db-4de2-aefd-ef30cedb0be1", "uri": "../unitgroups/1ebf3012-d0db-4de2-aefd-ef30cedb0be1"}}]}}, {"referenceToLCIAMethodDataSet": {"shortDescription": [{"value": "Depletion potential of the stratospheric ozone layer (ODP)", "lang": "en"}, {"value": "Abbaupotenzial der stratosphärischen Ozonschicht (ODP)", "lang": "de"}], "type": "LCIA method data set", "refObjectId": "b5c629d6-def3-11e6-bf01-fe55135034f3", "version": "02.00.013", "uri": "http://lca.jrc.ec.europa.eu/lcainfohub/datasets/elcd/lciamethods/8b723200-3d8f-4eec-9e10-444edb029476.xml"}, "meanAmount": 0.0, "other": {"anies": [{"value": "8.12E-7", "module": "A1", "scenario": "Standard Scenario"}, {"value": "2.19E-7", "module": "A2", "scenario": "Standard Scenario"}, {"value": "1.17E-7", "module": "A3", "scenario": "Standard Scenario"}, {"value": "1.03E-7", "module": "A4", "scenario": "Standard Scenario"}, {"value": "3.59E-8", "module": "A5", "scenario": "Standard Scenario"}, {"value": "0.0", "module": "C1", "scenario": "Standard Scenario"}, {"value": "2.82E-8", "module": "C2", "scenario": "Standard Scenario"}, {"value": "7.19E-9", "module": "C3", "scenario": "Standard Scenario"}, {"value": "1.05E-9", "module": "C4", "scenario": "Standard Scenario"}, {"value": "-3.76E-7", "module": "D", "scenario": "Standard Scenario"}, {"name": "referenceToUnitGroupDataSet", "value": {"shortDescription": [{"value": "kg CFC 11-Äquiv."}], "type": "unit group data set", "refObjectId": "d9e957c9-7309-4474-bf3a-7777df6c4e5b", "uri": "../unitgroups/d9e957c9-7309-4474-bf3a-7777df6c4e5b"}}]}}, {"referenceToLCIAMethodDataSet": {"shortDescription": [{"value": "Photochemical Ozone Creation Potential (POCP)", "lang": "en"}, {"value": "Bildungspotenzial für troposphärisches Ozon (POCP)", "lang": "de"}], "type": "LCIA method data set", "refObjectId": "b5c610fe-def3-11e6-bf01-fe55135034f3", "version": "02.00.016", "uri": "http://lca.jrc.ec.europa.eu/lcainfohub/datasets/elcd/lciamethods/ec7836be-83eb-41da-bcda-1a6a3fe2d149.xml"}, "meanAmount": 0.0, "other": {"anies": [{"value": "0.0282", "module": "A1", "scenario": "Standard Scenario"}, {"value": "0.0064", "module": "A2", "scenario": "Standard Scenario"}, {"value": "0.00214", "module": "A3", "scenario": "Standard Scenario"}, {"value": "0.003", "module": "A4", "scenario": "Standard Scenario"}, {"value": "0.00121", "module": "A5", "scenario": "Standard Scenario"}, {"value": "0.0", "module": "C1", "scenario": "Standard Scenario"}, {"value": "8.23E-4", "module": "C2", "scenario": "Standard Scenario"}, {"value": "0.00267", "module": "C3", "scenario": "Standard Scenario"}, {"value": "3.9E-5", "module": "C4", "scenario": "Standard Scenario"}, {"value": "-0.00511", "module": "D", "scenario": "Standard Scenario"}, {"name": "referenceToUnitGroupDataSet", "value": {"shortDescription": [{"value": "kg NMVOC eqv."}], "type": "unit group data set", "refObjectId": "d27c25f8-fbc1-44c6-b47b-4adbae4199c6", "uri": "../unitgroups/d27c25f8-fbc1-44c6-b47b-4adbae4199c6"}}]}}, {"referenceToLCIAMethodDataSet": {"shortDescription": [{"value": "Water (user) deprivation potential (WDP)", "lang": "en"}, {"value": "Wasser-Entzugspotenzial (Benutzer) (WDP)", "lang": "de"}], "type": "LCIA method data set", "refObjectId": "b2ad66ce-c78d-11e6-9d9d-cec0c932ce01", "version": "03.00.015"}, "meanAmount": 0.0, "other": {"anies": [{"value": "6.4", "module": "A1", "scenario": "Standard Scenario"}, {"value": "0.0536", "module": "A2", "scenario": "Standard Scenario"}, {"value": "0.235", "module": "A3", "scenario": "Standard Scenario"}, {"value": "0.0252", "module": "A4", "scenario": "Standard Scenario"}, {"value": "0.202", "module": "A5", "scenario": "Standard Scenario"}, {"value": "0.0", "module": "C1", "scenario": "Standard Scenario"}, {"value": "0.0069", "module": "C2", "scenario": "Standard Scenario"}, {"value": "0.02", "module": "C3", "scenario": "Standard Scenario"}, {"value": "0.00345", "module": "C4", "scenario": "Standard Scenario"}, {"value": "-0.103", "module": "D", "scenario": "Standard Scenario"}, {"name": "referenceToUnitGroupDataSet", "value": {"shortDescription": [{"value": "m3 world eqv."}], "type": "unit group data set", "refObjectId": "6ae2df01-888e-46c8-b17d-49fa3869b476", "uri": "../unitgroups/6ae2df01-888e-46c8-b17d-49fa3869b476"}}]}}, {"referenceToLCIAMethodDataSet": {"shortDescription": [{"value": "Potential incidence of disease due to PM emissions (PM)", "lang": "en"}, {"value": "Potenzielles Auftreten von Krankheiten aufgrund von Feinstaubemissionen (PM)", "lang": "de"}], "type": "LCIA method data set", "refObjectId": "b5c602c6-def3-11e6-bf01-fe55135034f3", "version": "02.00.012", "uri": "http://lca.jrc.ec.europa.eu/lcainfohub/datasets/elcd/lciamethods/72ce3013-f678-4c6a-935b-f4752ff8901b.xml"}, "meanAmount": 0.0, "other": {"anies": [{"value": "5.78E-7", "module": "A1", "scenario": "Standard Scenario"}, {"value": "8.94E-8", "module": "A2", "scenario": "Standard Scenario"}, {"value": "2.74E-8", "module": "A3", "scenario": "Standard Scenario"}, {"value": "4.2E-8", "module": "A4", "scenario": "Standard Scenario"}, {"value": "2.17E-8", "module": "A5", "scenario": "Standard Scenario"}, {"value": "0.0", "module": "C1", "scenario": "Standard Scenario"}, {"value": "1.15E-8", "module": "C2", "scenario": "Standard Scenario"}, {"value": "1.54E-8", "module": "C3", "scenario": "Standard Scenario"}, {"value": "5.6E-10", "module": "C4", "scenario": "Standard Scenario"}, {"value": "-3.1E-8", "module": "D", "scenario": "Standard Scenario"}, {"name": "referenceToUnitGroupDataSet", "value": {"shortDescription": [{"value": "disease incidence"}], "type": "unit group data set", "refObjectId": "3883559b-648f-4afc-8ba2-0bd24f3affa3", "uri": "../unitgroups/3883559b-648f-4afc-8ba2-0bd24f3affa3"}}]}}, {"referenceToLCIAMethodDataSet": {"shortDescription": [{"value": "Potential Human exposure efficiency relative to U235 (IRP)", "lang": "en"}, {"value": "Potenzielle Wirkung durch Exposition des Menschen mit U235 (IRP)", "lang": "de"}], "type": "LCIA method data set", "refObjectId": "b5c632be-def3-11e6-bf01-fe55135034f3", "version": "01.00.012", "uri": "http://lca.jrc.ec.europa.eu/lcainfohub/datasets/elcd/lciamethods/a6f4cbc8-5388-44d6-9a67-53d05684f93e.xml"}, "meanAmount": 0.0, "other": {"anies": [{"value": "0.29", "module": "A1", "scenario": "Standard Scenario"}, {"value": "0.0628", "module": "A2", "scenario": "Standard Scenario"}, {"value": "0.0209", "module": "A3", "scenario": "Standard Scenario"}, {"value": "0.0295", "module": "A4", "scenario": "Standard Scenario"}, {"value": "0.0116", "module": "A5", "scenario": "Standard Scenario"}, {"value": "0.0", "module": "C1", "scenario": "Standard Scenario"}, {"value": "0.00808", "module": "C2", "scenario": "Standard Scenario"}, {"value": "0.00148", "module": "C3", "scenario": "Standard Scenario"}, {"value": "3.15E-4", "module": "C4", "scenario": "Standard Scenario"}, {"value": "-0.132", "module": "D", "scenario": "Standard Scenario"}, {"name": "referenceToUnitGroupDataSet", "value": {"shortDescription": [{"value": "kBq U235 eqv."}], "type": "unit group data set", "refObjectId": "456b05bf-1415-44a9-9993-02452f554c09", "uri": "../unitgroups/456b05bf-1415-44a9-9993-02452f554c09"}}]}}, {"referenceToLCIAMethodDataSet": {"shortDescription": [{"value": "Potential Comparative Toxic Unit for ecosystems (ETP-fw)", "lang": "en"}, {"value": "Potenzielle Toxizitätsvergleichseinheit für Ökosysteme (ETP-fw)", "lang": "de"}], "type": "LCIA method data set", "refObjectId": "ee1082d1-b0f7-43ca-a1f0-21e2a4a74511", "version": "01.00.003", "uri": "http://lca.jrc.ec.europa.eu/lcainfohub/datasets/elcd/lciamethods/ee1082d1-b0f7-43ca-a1f0-21e2a4a74511.xml"}, "meanAmount": 0.0, "other": {"anies": [{"value": "210.0", "module": "A1", "scenario": "Standard Scenario"}, {"value": "13.4", "module": "A2", "scenario": "Standard Scenario"}, {"value": "11.6", "module": "A3", "scenario": "Standard Scenario"}, {"value": "6.28", "module": "A4", "scenario": "Standard Scenario"}, {"value": "7.18", "module": "A5", "scenario": "Standard Scenario"}, {"value": "0.0", "module": "C1", "scenario": "Standard Scenario"}, {"value": "1.72", "module": "C2", "scenario": "Standard Scenario"}, {"value": "1.66", "module": "C3", "scenario": "Standard Scenario"}, {"value": "0.0807", "module": "C4", "scenario": "Standard Scenario"}, {"value": "-25.4", "module": "D", "scenario": "Standard Scenario"}, {"name": "referenceToUnitGroupDataSet", "value": {"shortDescription": [{"value": "CTUe"}], "type": "unit group data set", "refObjectId": "aa959ded-f1eb-4efb-9c5c-2d60be36b3e6", "uri": "../unitgroups/aa959ded-f1eb-4efb-9c5c-2d60be36b3e6"}}]}}, {"referenceToLCIAMethodDataSet": {"shortDescription": [{"value": "Potential Comparative Toxic Unit for humans - cancer effects (HTP-c)", "lang": "en"}, {"value": "Potenzielle Toxizitätsvergleichseinheit für den Menschen - kanzerogene Wirkung (HTP-c)", "lang": "de"}], "type": "LCIA method data set", "refObjectId": "2299222a-bbd8-474f-9d4f-4dd1f18aea7c", "version": "01.00.004", "uri": "http://lca.jrc.ec.europa.eu/lcainfohub/datasets/elcd/lciamethods/2299222a-bbd8-474f-9d4f-4dd1f18aea7c.xml"}, "meanAmount": 0.0, "other": {"anies": [{"value": "6.32E-8", "module": "A1", "scenario": "Standard Scenario"}, {"value": "4.34E-10", "module": "A2", "scenario": "Standard Scenario"}, {"value": "2.8E-9", "module": "A3", "scenario": "Standard Scenario"}, {"value": "2.04E-10", "module": "A4", "scenario": "Standard Scenario"}, {"value": "2.71E-9", "module": "A5", "scenario": "Standard Scenario"}, {"value": "0.0", "module": "C1", "scenario": "Standard Scenario"}, {"value": "5.58E-11", "module": "C2", "scenario": "Standard Scenario"}, {"value": "2.37E-8", "module": "C3", "scenario": "Standard Scenario"}, {"value": "2.24E-12", "module": "C4", "scenario": "Standard Scenario"}, {"value": "-5.76E-10", "module": "D", "scenario": "Standard Scenario"}, {"name": "referenceToUnitGroupDataSet", "value": {"shortDescription": [{"value": "CTUh"}], "type": "unit group data set", "refObjectId": "d4c9523e-2d7e-49fd-8469-998f547d3a70", "uri": "../unitgroups/d4c9523e-2d7e-49fd-8469-998f547d3a70"}}]}}, {"referenceToLCIAMethodDataSet": {"shortDescription": [{"value": "Potential Comparative Toxic Unit for humans - non-cancer effects (HTP-nc)", "lang": "en"}, {"value": "Potenzielle Toxizitätsvergleichseinheit für den Menschen - nicht kanzerogene Wirkung (HTP-nc)", "lang": "de"}], "type": "LCIA method data set", "refObjectId": "3af763a5-b7a1-48c9-9cee-1f223481fcef", "version": "01.00.003", "uri": "http://lca.jrc.ec.europa.eu/lcainfohub/datasets/elcd/lciamethods/3af763a5-b7a1-48c9-9cee-1f223481fcef.xml"}, "meanAmount": 0.0, "other": {"anies": [{"value": "2.31E-7", "module": "A1", "scenario": "Standard Scenario"}, {"value": "1.46E-8", "module": "A2", "scenario": "Standard Scenario"}, {"value": "1.04E-8", "module": "A3", "scenario": "Standard Scenario"}, {"value": "6.87E-9", "module": "A4", "scenario": "Standard Scenario"}, {"value": "7.94E-9", "module": "A5", "scenario": "Standard Scenario"}, {"value": "0.0", "module": "C1", "scenario": "Standard Scenario"}, {"value": "1.88E-9", "module": "C2", "scenario": "Standard Scenario"}, {"value": "5.82E-9", "module": "C3", "scenario": "Standard Scenario"}, {"value": "8.62E-11", "module": "C4", "scenario": "Standard Scenario"}, {"value": "-2.09E-8", "module": "D", "scenario": "Standard Scenario"}, {"name": "referenceToUnitGroupDataSet", "value": {"shortDescription": [{"value": "CTUh"}], "type": "unit group data set", "refObjectId": "d4c9523e-2d7e-49fd-8469-998f547d3a70", "uri": "../unitgroups/d4c9523e-2d7e-49fd-8469-998f547d3a70"}}]}}, {"referenceToLCIAMethodDataSet": {"shortDescription": [{"value": "Potential Soil quality index (SQP)", "lang": "en"}, {"value": "Potenzieller Bodenqualitätsindex (SQP)", "lang": "de"}], "type": "LCIA method data set", "refObjectId": "b2ad6890-c78d-11e6-9d9d-cec0c932ce01", "version": "01.00.011"}, "meanAmount": 0.0, "other": {"anies": [{"value": "404.0", "module": "A1", "scenario": "Standard Scenario"}, {"value": "13.0", "module": "A2", "scenario": "Standard Scenario"}, {"value": "27.3", "module": "A3", "scenario": "Standard Scenario"}, {"value": "6.11", "module": "A4", "scenario": "Standard Scenario"}, {"value": "13.4", "module": "A5", "scenario": "Standard Scenario"}, {"value": "0.0", "module": "C1", "scenario": "Standard Scenario"}, {"value": "1.67", "module": "C2", "scenario": "Standard Scenario"}, {"value": "0.198", "module": "C3", "scenario": "Standard Scenario"}, {"value": "0.191", "module": "C4", "scenario": "Standard Scenario"}, {"value": "-7.38", "module": "D", "scenario": "Standard Scenario"}, {"name": "referenceToUnitGroupDataSet", "value": {"shortDescription": [{"value": "dimensionless"}], "type": "unit group data set", "refObjectId": "f130951c-e67f-4f7f-8dd4-665de3974e18", "uri": "../unitgroups/f130951c-e67f-4f7f-8dd4-665de3974e18"}}]}}]}, "otherAttributes": {"{http://www.indata.network/EPD/2019}epd-version": "1.2", "{http://www.okworx.com/ILCD/Extensions/2018/Profile}profile": "EN_15804_A2"}, "version": "1.1"}