{"processInformation": {"dataSetInformation": {"UUID": "8a44cf09-80bf-44be-a021-3a3da720a26f", "name": {"baseName": [{"value": "Kaminsysteme – Schiedel – Edelstahl-Kaminsystem PRIMA PLUS (einwandig) ", "lang": "de"}, {"value": "Chimney systems - Schiedel - Stainless steel chimney system PRIMA PLUS (single-walled)", "lang": "en"}]}, "synonyms": [{"value": "Prima Smooth", "lang": "de"}, {"value": "Prima Smooth", "lang": "en"}], "classificationInformation": {"classification": [{"class": [{"value": "Gebäudetechnik", "level": 0, "classId": "8"}, {"value": "Heizung", "level": 1, "classId": "8.1"}, {"value": "Wärmeerzeuger", "level": 2, "classId": "8.1.01"}], "name": "OEKOBAU.DAT"}]}, "generalComment": [{"value": "\tCradle to Gate\r\nThis data set contains the results for modules A1-A3 and modules C1, C2, C3, C4, D. The environmental profile contains the expenses for the life cycle stages cradle to gate with options (modules A1-A3 + C + D). The production of packaging was taken into account within modules A1-A3\r\n\t\t\r\n\tCradle to Grave\r\nThis data set contains the results for modules A1-A3 and modules A4, A5, B1, B2, B3, B4, B5, B6, B7, C1, C2, C3, C4, D. The environmental profile contains the expenditure for the cradle to grave life cycle stages (modules A + B + C + D). The production of the packaging was taken into account within modules A1-A3.", "lang": "en"}, {"value": "Dieser Datensatz beinhaltet die Ergebnisse für die Module A1-A3 sowie Module A4, A5, B1, B2, B3, B4, B5, B6, B7, C1, C2, C3, C4, D. Das Umweltprofil beinhaltet die Aufwendungen für die Lebenszyklus-Stadien cradle to grave (Modul A + B + C + D). Die Herstellung der Verpackung wurde innerhalb der Module A1-A3 berücksichtigt. ", "lang": "de"}], "other": {"anies": [{"margins": 0.0}, "<ns11:modules xmlns:ns11=\"http://openlca.org/epd_ilcd\" xmlns=\"http://lca.jrc.it/ILCD/Process\" xmlns:c=\"http://lca.jrc.it/ILCD/Contact\" xmlns:common=\"http://lca.jrc.it/ILCD/Common\" xmlns:epd=\"http://www.iai.kit.edu/EPD/2013\" xmlns:epd2=\"http://www.indata.network/EPD/2019\" xmlns:f=\"http://lca.jrc.it/ILCD/Flow\" xmlns:fp=\"http://lca.jrc.it/ILCD/FlowProperty\" xmlns:m=\"http://lca.jrc.it/ILCD/LCIAMethod\" xmlns:ns9=\"http://www.okworx.com/ILCD/Extensions/2018/Profile\" xmlns:s=\"http://lca.jrc.it/ILCD/Source\" xmlns:u=\"http://lca.jrc.it/ILCD/UnitGroup\" name=\"A1-A3\"/>", "<ns11:modules xmlns:ns11=\"http://openlca.org/epd_ilcd\" xmlns=\"http://lca.jrc.it/ILCD/Process\" xmlns:c=\"http://lca.jrc.it/ILCD/Contact\" xmlns:common=\"http://lca.jrc.it/ILCD/Common\" xmlns:epd=\"http://www.iai.kit.edu/EPD/2013\" xmlns:epd2=\"http://www.indata.network/EPD/2019\" xmlns:f=\"http://lca.jrc.it/ILCD/Flow\" xmlns:fp=\"http://lca.jrc.it/ILCD/FlowProperty\" xmlns:m=\"http://lca.jrc.it/ILCD/LCIAMethod\" xmlns:ns9=\"http://www.okworx.com/ILCD/Extensions/2018/Profile\" xmlns:s=\"http://lca.jrc.it/ILCD/Source\" xmlns:u=\"http://lca.jrc.it/ILCD/UnitGroup\" name=\"A4\"/>", "<ns11:modules xmlns:ns11=\"http://openlca.org/epd_ilcd\" xmlns=\"http://lca.jrc.it/ILCD/Process\" xmlns:c=\"http://lca.jrc.it/ILCD/Contact\" xmlns:common=\"http://lca.jrc.it/ILCD/Common\" xmlns:epd=\"http://www.iai.kit.edu/EPD/2013\" xmlns:epd2=\"http://www.indata.network/EPD/2019\" xmlns:f=\"http://lca.jrc.it/ILCD/Flow\" xmlns:fp=\"http://lca.jrc.it/ILCD/FlowProperty\" xmlns:m=\"http://lca.jrc.it/ILCD/LCIAMethod\" xmlns:ns9=\"http://www.okworx.com/ILCD/Extensions/2018/Profile\" xmlns:s=\"http://lca.jrc.it/ILCD/Source\" xmlns:u=\"http://lca.jrc.it/ILCD/UnitGroup\" name=\"A5\"/>", "<ns11:modules xmlns:ns11=\"http://openlca.org/epd_ilcd\" xmlns=\"http://lca.jrc.it/ILCD/Process\" xmlns:c=\"http://lca.jrc.it/ILCD/Contact\" xmlns:common=\"http://lca.jrc.it/ILCD/Common\" xmlns:epd=\"http://www.iai.kit.edu/EPD/2013\" xmlns:epd2=\"http://www.indata.network/EPD/2019\" xmlns:f=\"http://lca.jrc.it/ILCD/Flow\" xmlns:fp=\"http://lca.jrc.it/ILCD/FlowProperty\" xmlns:m=\"http://lca.jrc.it/ILCD/LCIAMethod\" xmlns:ns9=\"http://www.okworx.com/ILCD/Extensions/2018/Profile\" xmlns:s=\"http://lca.jrc.it/ILCD/Source\" xmlns:u=\"http://lca.jrc.it/ILCD/UnitGroup\" name=\"B1\"/>", "<ns11:modules xmlns:ns11=\"http://openlca.org/epd_ilcd\" xmlns=\"http://lca.jrc.it/ILCD/Process\" xmlns:c=\"http://lca.jrc.it/ILCD/Contact\" xmlns:common=\"http://lca.jrc.it/ILCD/Common\" xmlns:epd=\"http://www.iai.kit.edu/EPD/2013\" xmlns:epd2=\"http://www.indata.network/EPD/2019\" xmlns:f=\"http://lca.jrc.it/ILCD/Flow\" xmlns:fp=\"http://lca.jrc.it/ILCD/FlowProperty\" xmlns:m=\"http://lca.jrc.it/ILCD/LCIAMethod\" xmlns:ns9=\"http://www.okworx.com/ILCD/Extensions/2018/Profile\" xmlns:s=\"http://lca.jrc.it/ILCD/Source\" xmlns:u=\"http://lca.jrc.it/ILCD/UnitGroup\" name=\"B2\"/>", "<ns11:modules xmlns:ns11=\"http://openlca.org/epd_ilcd\" xmlns=\"http://lca.jrc.it/ILCD/Process\" xmlns:c=\"http://lca.jrc.it/ILCD/Contact\" xmlns:common=\"http://lca.jrc.it/ILCD/Common\" xmlns:epd=\"http://www.iai.kit.edu/EPD/2013\" xmlns:epd2=\"http://www.indata.network/EPD/2019\" xmlns:f=\"http://lca.jrc.it/ILCD/Flow\" xmlns:fp=\"http://lca.jrc.it/ILCD/FlowProperty\" xmlns:m=\"http://lca.jrc.it/ILCD/LCIAMethod\" xmlns:ns9=\"http://www.okworx.com/ILCD/Extensions/2018/Profile\" xmlns:s=\"http://lca.jrc.it/ILCD/Source\" xmlns:u=\"http://lca.jrc.it/ILCD/UnitGroup\" name=\"B3\"/>", "<ns11:modules xmlns:ns11=\"http://openlca.org/epd_ilcd\" xmlns=\"http://lca.jrc.it/ILCD/Process\" xmlns:c=\"http://lca.jrc.it/ILCD/Contact\" xmlns:common=\"http://lca.jrc.it/ILCD/Common\" xmlns:epd=\"http://www.iai.kit.edu/EPD/2013\" xmlns:epd2=\"http://www.indata.network/EPD/2019\" xmlns:f=\"http://lca.jrc.it/ILCD/Flow\" xmlns:fp=\"http://lca.jrc.it/ILCD/FlowProperty\" xmlns:m=\"http://lca.jrc.it/ILCD/LCIAMethod\" xmlns:ns9=\"http://www.okworx.com/ILCD/Extensions/2018/Profile\" xmlns:s=\"http://lca.jrc.it/ILCD/Source\" xmlns:u=\"http://lca.jrc.it/ILCD/UnitGroup\" name=\"B4\"/>", "<ns11:modules xmlns:ns11=\"http://openlca.org/epd_ilcd\" xmlns=\"http://lca.jrc.it/ILCD/Process\" xmlns:c=\"http://lca.jrc.it/ILCD/Contact\" xmlns:common=\"http://lca.jrc.it/ILCD/Common\" xmlns:epd=\"http://www.iai.kit.edu/EPD/2013\" xmlns:epd2=\"http://www.indata.network/EPD/2019\" xmlns:f=\"http://lca.jrc.it/ILCD/Flow\" xmlns:fp=\"http://lca.jrc.it/ILCD/FlowProperty\" xmlns:m=\"http://lca.jrc.it/ILCD/LCIAMethod\" xmlns:ns9=\"http://www.okworx.com/ILCD/Extensions/2018/Profile\" xmlns:s=\"http://lca.jrc.it/ILCD/Source\" xmlns:u=\"http://lca.jrc.it/ILCD/UnitGroup\" name=\"B5\"/>", "<ns11:modules xmlns:ns11=\"http://openlca.org/epd_ilcd\" xmlns=\"http://lca.jrc.it/ILCD/Process\" xmlns:c=\"http://lca.jrc.it/ILCD/Contact\" xmlns:common=\"http://lca.jrc.it/ILCD/Common\" xmlns:epd=\"http://www.iai.kit.edu/EPD/2013\" xmlns:epd2=\"http://www.indata.network/EPD/2019\" xmlns:f=\"http://lca.jrc.it/ILCD/Flow\" xmlns:fp=\"http://lca.jrc.it/ILCD/FlowProperty\" xmlns:m=\"http://lca.jrc.it/ILCD/LCIAMethod\" xmlns:ns9=\"http://www.okworx.com/ILCD/Extensions/2018/Profile\" xmlns:s=\"http://lca.jrc.it/ILCD/Source\" xmlns:u=\"http://lca.jrc.it/ILCD/UnitGroup\" name=\"B6\"/>", "<ns11:modules xmlns:ns11=\"http://openlca.org/epd_ilcd\" xmlns=\"http://lca.jrc.it/ILCD/Process\" xmlns:c=\"http://lca.jrc.it/ILCD/Contact\" xmlns:common=\"http://lca.jrc.it/ILCD/Common\" xmlns:epd=\"http://www.iai.kit.edu/EPD/2013\" xmlns:epd2=\"http://www.indata.network/EPD/2019\" xmlns:f=\"http://lca.jrc.it/ILCD/Flow\" xmlns:fp=\"http://lca.jrc.it/ILCD/FlowProperty\" xmlns:m=\"http://lca.jrc.it/ILCD/LCIAMethod\" xmlns:ns9=\"http://www.okworx.com/ILCD/Extensions/2018/Profile\" xmlns:s=\"http://lca.jrc.it/ILCD/Source\" xmlns:u=\"http://lca.jrc.it/ILCD/UnitGroup\" name=\"B7\"/>", "<ns11:modules xmlns:ns11=\"http://openlca.org/epd_ilcd\" xmlns=\"http://lca.jrc.it/ILCD/Process\" xmlns:c=\"http://lca.jrc.it/ILCD/Contact\" xmlns:common=\"http://lca.jrc.it/ILCD/Common\" xmlns:epd=\"http://www.iai.kit.edu/EPD/2013\" xmlns:epd2=\"http://www.indata.network/EPD/2019\" xmlns:f=\"http://lca.jrc.it/ILCD/Flow\" xmlns:fp=\"http://lca.jrc.it/ILCD/FlowProperty\" xmlns:m=\"http://lca.jrc.it/ILCD/LCIAMethod\" xmlns:ns9=\"http://www.okworx.com/ILCD/Extensions/2018/Profile\" xmlns:s=\"http://lca.jrc.it/ILCD/Source\" xmlns:u=\"http://lca.jrc.it/ILCD/UnitGroup\" name=\"C1\"/>", "<ns11:modules xmlns:ns11=\"http://openlca.org/epd_ilcd\" xmlns=\"http://lca.jrc.it/ILCD/Process\" xmlns:c=\"http://lca.jrc.it/ILCD/Contact\" xmlns:common=\"http://lca.jrc.it/ILCD/Common\" xmlns:epd=\"http://www.iai.kit.edu/EPD/2013\" xmlns:epd2=\"http://www.indata.network/EPD/2019\" xmlns:f=\"http://lca.jrc.it/ILCD/Flow\" xmlns:fp=\"http://lca.jrc.it/ILCD/FlowProperty\" xmlns:m=\"http://lca.jrc.it/ILCD/LCIAMethod\" xmlns:ns9=\"http://www.okworx.com/ILCD/Extensions/2018/Profile\" xmlns:s=\"http://lca.jrc.it/ILCD/Source\" xmlns:u=\"http://lca.jrc.it/ILCD/UnitGroup\" name=\"C2\"/>", "<ns11:modules xmlns:ns11=\"http://openlca.org/epd_ilcd\" xmlns=\"http://lca.jrc.it/ILCD/Process\" xmlns:c=\"http://lca.jrc.it/ILCD/Contact\" xmlns:common=\"http://lca.jrc.it/ILCD/Common\" xmlns:epd=\"http://www.iai.kit.edu/EPD/2013\" xmlns:epd2=\"http://www.indata.network/EPD/2019\" xmlns:f=\"http://lca.jrc.it/ILCD/Flow\" xmlns:fp=\"http://lca.jrc.it/ILCD/FlowProperty\" xmlns:m=\"http://lca.jrc.it/ILCD/LCIAMethod\" xmlns:ns9=\"http://www.okworx.com/ILCD/Extensions/2018/Profile\" xmlns:s=\"http://lca.jrc.it/ILCD/Source\" xmlns:u=\"http://lca.jrc.it/ILCD/UnitGroup\" name=\"C3\"/>", "<ns11:modules xmlns:ns11=\"http://openlca.org/epd_ilcd\" xmlns=\"http://lca.jrc.it/ILCD/Process\" xmlns:c=\"http://lca.jrc.it/ILCD/Contact\" xmlns:common=\"http://lca.jrc.it/ILCD/Common\" xmlns:epd=\"http://www.iai.kit.edu/EPD/2013\" xmlns:epd2=\"http://www.indata.network/EPD/2019\" xmlns:f=\"http://lca.jrc.it/ILCD/Flow\" xmlns:fp=\"http://lca.jrc.it/ILCD/FlowProperty\" xmlns:m=\"http://lca.jrc.it/ILCD/LCIAMethod\" xmlns:ns9=\"http://www.okworx.com/ILCD/Extensions/2018/Profile\" xmlns:s=\"http://lca.jrc.it/ILCD/Source\" xmlns:u=\"http://lca.jrc.it/ILCD/UnitGroup\" name=\"C4\"/>", "<ns11:modules xmlns:ns11=\"http://openlca.org/epd_ilcd\" xmlns=\"http://lca.jrc.it/ILCD/Process\" xmlns:c=\"http://lca.jrc.it/ILCD/Contact\" xmlns:common=\"http://lca.jrc.it/ILCD/Common\" xmlns:epd=\"http://www.iai.kit.edu/EPD/2013\" xmlns:epd2=\"http://www.indata.network/EPD/2019\" xmlns:f=\"http://lca.jrc.it/ILCD/Flow\" xmlns:fp=\"http://lca.jrc.it/ILCD/FlowProperty\" xmlns:m=\"http://lca.jrc.it/ILCD/LCIAMethod\" xmlns:ns9=\"http://www.okworx.com/ILCD/Extensions/2018/Profile\" xmlns:s=\"http://lca.jrc.it/ILCD/Source\" xmlns:u=\"http://lca.jrc.it/ILCD/UnitGroup\" name=\"D\"/>"]}}, "quantitativeReference": {"referenceToReferenceFlow": [1], "type": "Reference flow(s)"}, "time": {"referenceYear": 2025, "dataSetValidUntil": 2030, "timeRepresentativenessDescription": [{"value": "jährlicher Durchschnitt", "lang": "de"}, {"value": "annual average", "lang": "en"}], "other": {"anies": [{"name": "publicationDateOfEPD", "value": 1761782400000}]}}, "geography": {"locationOfOperationSupplyOrProduction": {"descriptionOfRestrictions": [{"value": "Dieser Datensatz repräsentiert die Situation des Unternehmens Schiedel s.r.o., 415 02 Teplice (CZ) im Hinblick auf die wichtigsten Technologien und die gesetzlichen Rahmenbedingungen.", "lang": "de"}, {"value": "This data set represents the situation of the company Schiedel s.r.o., 415 02 Teplice (CZ) with regard to the most important technologies and the legal framework.", "lang": "en"}], "location": "CZ"}}, "technology": {"technologyDescriptionAndIncludedProcesses": [{"value": "Die Ökobilanzergebnisse umfassen die Lebenszyklusstadien der Herstellung der Vorprodukte bis hin zur Rohstoffgewinnung und Verarbeitungsprozesse von als Input dienenden Sekundärstoffen (z.B. Recyclingprozesse), deren Transporte zum Werk sowie die Produktion selbst, einschließlich der Bereitstellung von allen Hilfs- und Betriebsstoffen, Energie, sowie die vollständige Abfallbehandlung oder die Deponierung der Restabfälle während des Stadiums der Produktion. Die Module A1, A2 und A3 sind hier als ein aggregiertes Modul A1-A3 ausgewiesen. Falls für diesen Datensatz weitere Module berechnet wurden, sind diese separat zu finden und können für eine Betrachtung des gesamten Lebenszyklus zusammengeführt werden.", "lang": "de"}, {"value": "The life cycle assessment results cover the life cycle stages from the manufacture of primary products to the extraction of raw materials and processing of secondary materials used as input (e.g. recycling processes), their transportation to the plant and the production itself, including the provision of all auxiliary and operating materials, energy, as well as the complete waste treatment or landfilling of residual waste during the production stage. Modules A1, A2 and A3 are shown here as an aggregated module A1-A3. If further modules were calculated for this data set, these can be found separately and can be combined for a consideration of the entire life cycle.", "lang": "en"}], "technologicalApplicability": [{"value": "Prima Plus:\r\nEinwandige Edelstahl-Abgasleitung zur Sanierung von bestehenden Schornsteinen \r\n●\tfür die Herstellung von Verbindungsleitungen,\r\n●\tfür alle Brennstoffe und Heizgerätetypen geeignet,\r\n●\tfür den Einsatz bei hohen und niedrigen Abgastemperaturen, \r\n●\tim Über- und Unterdruck\r\n\r\nEinwandige Edelstahl-Abgasleitung, erhältlich in den Durchmessern von 80 bis 1200 mm, die Elemente bestehen aus Edelstahl 1.4404 in einer Wandstärke von 0,6 bis 1,0 mm. Es ist im Unterdruck bis zu Abgastemperaturen bis 600 °C einsetzbar und rußbrandbeständig. Bei Temperaturen bis 200 °C ist es durch Silikondichtungen an den Verbindungen für Überdrück bis 200 Pa einsetzbar.\r\n", "lang": "de"}, {"value": "Prima Plus:\r\nSingle-walled stainless steel flue pipe for renovating existing chimneys\r\n•\tfor manufacturing connecting pipes,\r\n•\tsuitable for all fuels and types of heating appliances,\r\n•\tfor use with high and low flue gas temperatures,\r\n•\tin positive and negative pressure\r\n\r\nSingle-walled stainless steel exhaust pipe, available in diameters from 80 to 1200 mm, the elements are made of 1.4404 stainless steel with a wall thickness of 0.6 to 1.0 mm. It can be used in negative pressure up to exhaust gas temperatures of 600 °C and is resistant to soot fires. At temperatures up to 200 °C, it can be used for overpressure up to 200 Pa thanks to silicone seals at the connections.\r\n\r\nFor a detailed product description refer to the manufacturer specifications or the product specifications of the respective offer/quotation.\r\n", "lang": "en"}]}}, "modellingAndValidation": {"LCIMethodAndAllocation": {"typeOfDataSet": "EPD", "referenceToLCAMethodDetails": [{"shortDescription": [{"value": "Produktkategorieregeln Teil A", "lang": "de"}, {"value": "Product category rules Part A", "lang": "en"}], "type": "source data set", "refObjectId": "c6e986be-62a9-4f2f-b486-27aa9129eaeb", "version": "00.00.014"}, {"shortDescription": [{"value": "Produktkategorieregeln Teil B – für Rohrleitungssysteme einschließlich Verbindungs- und Anschlusstechnik", "lang": "de"}, {"value": "Product category rules Part B – for piping systems including joining and connection technology", "lang": "en"}], "type": "source data set", "refObjectId": "7e9eab7f-c1ac-43ac-84f1-4f240c75d7f7", "version": "00.00.007"}], "other": {"anies": [{"name": "subType", "value": "specific dataset"}]}}, "dataSourcesTreatmentAndRepresentativeness": {"referenceToDataSource": [{"shortDescription": [{"value": "GaBi database (general)", "lang": "en"}], "type": "source data set", "refObjectId": "28d74cc0-db8b-4d7e-bc44-5f6d56ce0c4a", "version": "00.03.003"}], "useAdviceForDataSet": [{"value": "This data set contains the results for modules A1-A3 as well as modules A4, A5, B1, B2, B3, B4, B5, B6, B7, C1, C2, C3, C4 and D in accordance with EN 15804 + A2. \nThe modeling of the B-modules was based on 1 year.\nA comparison with other products is only permissible with a comparable application in the building. In principle, a comparison or evaluation of EPD data is only possible if all data sets to be compared were created in accordance with EN 15804 + A2 and the building context or the product-specific performance characteristics are taken into account.", "lang": "en"}, {"value": "Dieser Datensatz beinhaltet die Ergebnisse für die Module A1-A3 sowie die Module A4, A5, B1, B2, B3, B4, B5, B6, B7, C1, C2, C3, C4 und D gemäß EN 15804 + A2. Die Modellierung der B-Module wurde bezogen auf 1 Jahr vorgenommen.\r\nEin Vergleich mit anderen Produkten ist nur mit einer vergleichbaren Anwendung im Gebäude zulässig. Grundsätzlich ist eine Gegenüberstellung oder die Bewertung von EPD Daten nur möglich, wenn alle zu vergleichenden Datensätze nach EN 15804 + A2 erstellt wurden und der Gebäudekontext, bzw. die produktspezifischen Leistungsmerkmale berücksichtigt werden.", "lang": "de"}], "other": {"anies": [{"name": "referenceToOriginalEPD", "value": {"shortDescription": {"value": "EPD - Kaminsysteme - Schiedel - Edelstahl-Kaminsysteme", "defaultValue": "EPD - Kaminsysteme - Schiedel - Edelstahl-Kaminsysteme", "lstrings": [{"lang": "de", "value": "EPD - Kaminsysteme - Schiedel - Edelstahl-Kaminsysteme"}, {"lang": "en", "value": "EPD - Chimney systems - Schiedel - Stainless steel chimney systems"}]}, "version": {"version": 5, "majorVersion": 0, "minorVersion": 0, "subMinorVersion": 5, "zero": false, "versionString": "00.00.005"}, "type": "source data set", "uuid": {"uuid": "b958e9a2-e495-43ee-881a-7bd59c268e58"}, "refObjectId": "b958e9a2-e495-43ee-881a-7bd59c268e58", "versionAsString": "00.00.005", "resourceURLs": ["https://oekobaudat.de/OEKOBAU.DAT/resource/sources/b958e9a2-e495-43ee-881a-7bd59c268e58/EPD-SEK-GB-97.0.pdf?version=00.00.005", "https://oekobaudat.de/OEKOBAU.DAT/resource/sources/b958e9a2-e495-43ee-881a-7bd59c268e58/EPD-SEK-97.0.pdf?version=00.00.005"]}}]}}, "validation": {"review": [{"reviewDetails": [{"value": "Die angewendete LCI Methode ist in Übereinstimmung mit ISO 14040 und 14044. Die Dokumentation enthält alle relevanten Informationen im Hinblick auf die Datenqualität und den Umfang der Anwendung der jeweiligen LCI Ergebnisse bzw. der Datensätze. Der Datensatz repräsentiert den Stand der Technik bezogen auf die funktionelle Einheit.", "lang": "de"}, {"value": "The LCI method used is in accordance with ISO 14040 and 14044. The documentation contains all relevant information with regard to the data quality and the scope of application of the respective LCI results or data sets. The data set represents the state of the art in relation to the functional unit.", "lang": "en"}], "referenceToNameOfReviewerAndInstitution": [{"shortDescription": [{"value": "Eric Brehm", "lang": "de"}], "type": "contact data set", "refObjectId": "ef2baa7d-04f8-424a-af3d-38561f10b8d1", "version": "00.00.001"}], "type": "Independent external review"}]}, "complianceDeclarations": {"compliance": [{"referenceToComplianceSystem": {"shortDescription": [{"value": "EN 15804+A2 (EF 3.1)", "lang": "de"}, {"value": "EN 15804+A2 (EF 3.1)", "lang": "en"}], "type": "source data set", "refObjectId": "d4aa3ec7-b1d7-4a4a-a6cb-37af88dcc902", "version": "00.01.000"}}]}}, "administrativeInformation": {"dataGenerator": {"referenceToPersonOrEntityGeneratingTheDataSet": [{"shortDescription": [{"value": "ift Rosenheim", "lang": "de"}], "type": "contact data set", "refObjectId": "bdf65bd4-c474-4c23-8269-124ba43fa2b9", "version": "25.00.004"}]}, "dataEntryBy": {"timeStamp": 1761822064873, "referenceToDataSetFormat": [{"shortDescription": [{"value": "EPD Data Format Extensions v1.2", "lang": "en"}, {"value": "EPD-Datenformaterweiterungen v1.2", "lang": "de"}], "type": "source data set", "refObjectId": "a29449fd-aa2f-4de8-b5d7-4b06b43c6fde", "version": "00.01.003"}, {"shortDescription": [{"value": "ILCD format", "lang": "en"}], "type": "source data set", "refObjectId": "a97a0155-0234-4b87-b4ce-a45da52f2a40", "version": "03.01.004", "uri": "http://lca.jrc.ec.europa.eu/lcainfohub/datasets/ilcd/sources/a97a0155-0234-4b87-b4ce-a45da52f2a40.xml"}], "referenceToPersonOrEntityEnteringTheData": {"shortDescription": [{"value": "ift Rosenheim", "lang": "de"}], "type": "contact data set", "refObjectId": "bdf65bd4-c474-4c23-8269-124ba43fa2b9", "version": "25.00.004"}}, "publicationAndOwnership": {"dataSetVersion": "00.00.014", "referenceToRegistrationAuthority": {"shortDescription": [{"value": "ift Rosenheim", "lang": "de"}], "type": "contact data set", "refObjectId": "bdf65bd4-c474-4c23-8269-124ba43fa2b9", "version": "25.00.004"}, "registrationNumber": "EPD-SEK-97.0", "referenceToOwnershipOfDataSet": {"shortDescription": [{"value": "Schiedel s.r.o.", "lang": "de"}, {"value": "Schiedel s.r.o.", "lang": "en"}], "type": "contact data set", "refObjectId": "e85656db-acb7-4d4d-b374-4bcdca8d1f21", "version": "00.00.002"}, "copyright": true, "licenseType": "Free of charge for all users and uses", "accessRestrictions": [{"value": "none", "lang": "en"}, {"value": "keine", "lang": "de"}], "other": {"anies": [{"name": "referenceToPublisher", "value": {"shortDescription": [{"value": "ift Rosenheim", "lang": "de"}], "type": "contact data set", "refObjectId": "bdf65bd4-c474-4c23-8269-124ba43fa2b9", "version": "25.00.004"}}]}}}, "exchanges": {"exchange": [{"dataSetInternalID": 1, "referenceToFlowDataSet": {"shortDescription": [{"value": "Kaminsysteme - Schiedel - Edelstahl-Kaminsystem, einwandig", "lang": "de"}, {"value": "Chimney systems - Schiedel - Stainless steel chimney systems, single-walled", "lang": "en"}], "type": "flow data set", "refObjectId": "401ff07e-7e01-486b-90c6-aa90e259694d", "version": "00.00.005"}, "meanAmount": 1.0, "resultingAmount": 1.0, "referenceFlow": true, "resultingflowAmount": 1.0, "flowProperties": [{"name": [{"lang": "en", "value": "Carbon content (biogenic) - packaging"}], "uuid": "262a541b-209e-44cc-a426-33bce30de7b1", "meanValue": 0.46}, {"name": [{"lang": "de", "value": "Länge"}, {"lang": "en", "value": "Length"}], "uuid": "838aaa23-0117-11db-92e3-0800200c9a66", "referenceFlowProperty": true, "meanValue": 1.0, "referenceUnit": "m", "unitGroupUUID": "838aaa22-0117-11db-92e3-0800200c9a66"}, {"name": [{"lang": "en", "value": "Carbon content (biogenic)"}], "uuid": "62e503ce-544a-4599-b2ad-bcea15a7bf20", "meanValue": 0.0}], "materialProperties": [{"name": "diameter", "value": "150.0", "unit": "mm", "unitDescription": "diameter"}, {"name": "linear density", "value": "2.97", "unit": "kg/m"}], "typeOfFlow": "Product flow", "classification": {"classHierarchy": "Gebäudetechnik / Heizung / Wärmeerzeuger", "name": "OEKOBAU.DAT"}}, {"dataSetInternalID": 2, "referenceToFlowDataSet": {"shortDescription": [{"value": "Components for re-use (CRU)", "lang": "en"}, {"value": "Komponenten für die Wiederverwendung (CRU)", "lang": "de"}, {"value": "Componentes para su reutilización (CRU)", "lang": "es"}], "type": "flow data set", "refObjectId": "a2b32f97-3fc7-4af2-b209-525bc6426f33", "version": "30.00.000", "uri": "../flows/a2b32f97-3fc7-4af2-b209-525bc6426f33.xml"}, "exchange direction": "OUTPUT", "meanAmount": 0.0, "other": {"anies": [{"value": "0.0", "module": "A1-A3"}, {"value": "0.0", "module": "A4"}, {"value": "0.0", "module": "A5"}, {"value": "0.0", "module": "B1"}, {"value": "0.0", "module": "B2"}, {"value": "0.0", "module": "B3"}, {"value": "0.0", "module": "B4"}, {"value": "0.0", "module": "B5"}, {"value": "0.0", "module": "B6"}, {"value": "0.0", "module": "B7"}, {"value": "0.0", "module": "C1"}, {"value": "0.0", "module": "C2"}, {"value": "0.0", "module": "C3"}, {"value": "0.0", "module": "C4"}, {"value": "0.0", "module": "D"}, {"name": "referenceToUnitGroupDataSet", "value": {"shortDescription": [{"value": "kg", "lang": "en"}], "type": "unit group data set", "refObjectId": "ad38d542-3fe9-439d-9b95-2f5f7752acaf", "version": "30.00.000", "uri": "../unitgroups/ad38d542-3fe9-439d-9b95-2f5f7752acaf.xml"}}]}, "flowProperties": [], "typeOfFlow": "Other flow", "classification": {"classHierarchy": "Größen / Umweltliche Größen / EPD EN 15804 / LCI Indikatoren", "name": "GaBiCategories"}}, {"dataSetInternalID": 3, "referenceToFlowDataSet": {"shortDescription": [{"value": "Exported electrical energy (EEE)", "lang": "en"}, {"value": "Exportierte elektrische Energie (EEE)", "lang": "de"}, {"value": "Energía exportada electrica (EEE)", "lang": "es"}], "type": "flow data set", "refObjectId": "4da0c987-2b76-40d6-9e9e-82a017aaaf29", "version": "30.00.000", "uri": "../flows/4da0c987-2b76-40d6-9e9e-82a017aaaf29.xml"}, "exchange direction": "OUTPUT", "meanAmount": 0.0, "other": {"anies": [{"value": "0.44", "module": "A1-A3"}, {"value": "0.0", "module": "A4"}, {"value": "2.96", "module": "A5"}, {"value": "0.0", "module": "B1"}, {"value": "0.0", "module": "B2"}, {"value": "0.0", "module": "B3"}, {"value": "0.0697", "module": "B4"}, {"value": "0.0", "module": "B5"}, {"value": "0.0", "module": "B6"}, {"value": "0.0", "module": "B7"}, {"value": "0.0", "module": "C1"}, {"value": "0.0", "module": "C2"}, {"value": "0.0821", "module": "C3"}, {"value": "0.0", "module": "C4"}, {"value": "0.0", "module": "D"}, {"name": "referenceToUnitGroupDataSet", "value": {"shortDescription": [{"value": "MJ", "lang": "en"}], "type": "unit group data set", "refObjectId": "93a60a57-a3c8-11da-a746-0800200c9a66", "version": "03.00.000", "uri": "../unitgroups/93a60a57-a3c8-11da-a746-0800200c9a66.xml"}}]}, "flowProperties": [], "typeOfFlow": "Other flow", "classification": {"classHierarchy": "Größen / Umweltliche Größen / EPD EN 15804 / LCI Indikatoren", "name": "GaBiCategories"}}, {"dataSetInternalID": 4, "referenceToFlowDataSet": {"shortDescription": [{"value": "Exported thermal energy (EET)", "lang": "en"}, {"value": "Exportierte thermische Energie (EET)", "lang": "de"}, {"value": "Energía exportada termal (EET)", "lang": "es"}], "type": "flow data set", "refObjectId": "98daf38a-7a79-46d3-9a37-2b7bd0955810", "version": "30.00.000", "uri": "../flows/98daf38a-7a79-46d3-9a37-2b7bd0955810.xml"}, "exchange direction": "OUTPUT", "meanAmount": 0.0, "other": {"anies": [{"value": "0.8", "module": "A1-A3"}, {"value": "0.0", "module": "A4"}, {"value": "5.37", "module": "A5"}, {"value": "0.0", "module": "B1"}, {"value": "0.0", "module": "B2"}, {"value": "0.0", "module": "B3"}, {"value": "0.13", "module": "B4"}, {"value": "0.0", "module": "B5"}, {"value": "0.0", "module": "B6"}, {"value": "0.0", "module": "B7"}, {"value": "0.0", "module": "C1"}, {"value": "0.0", "module": "C2"}, {"value": "0.19", "module": "C3"}, {"value": "0.0", "module": "C4"}, {"value": "0.0", "module": "D"}, {"name": "referenceToUnitGroupDataSet", "value": {"shortDescription": [{"value": "MJ", "lang": "en"}], "type": "unit group data set", "refObjectId": "93a60a57-a3c8-11da-a746-0800200c9a66", "version": "03.00.000", "uri": "../unitgroups/93a60a57-a3c8-11da-a746-0800200c9a66.xml"}}]}, "flowProperties": [], "typeOfFlow": "Other flow", "classification": {"classHierarchy": "Größen / Umweltliche Größen / EPD EN 15804 / LCI Indikatoren", "name": "GaBiCategories"}}, {"dataSetInternalID": 5, "referenceToFlowDataSet": {"shortDescription": [{"value": "Use of net fresh water (FW)", "lang": "en"}, {"value": "Einsatz von Süßwasserressourcen (FW)", "lang": "de"}, {"value": "Uso neto de recursos de agua dulce (FW)", "lang": "es"}], "type": "flow data set", "refObjectId": "3cf952c8-f3a4-461d-8c96-96456ca62246", "version": "30.00.000", "uri": "../flows/3cf952c8-f3a4-461d-8c96-96456ca62246.xml"}, "exchange direction": "INPUT", "meanAmount": 0.0, "other": {"anies": [{"value": "0.26", "module": "A1-A3"}, {"value": "5.16E-4", "module": "A4"}, {"value": "0.0056", "module": "A5"}, {"value": "0.0", "module": "B1"}, {"value": "0.0", "module": "B2"}, {"value": "0.0", "module": "B3"}, {"value": "0.00373", "module": "B4"}, {"value": "0.0", "module": "B5"}, {"value": "0.0", "module": "B6"}, {"value": "0.0", "module": "B7"}, {"value": "0.0", "module": "C1"}, {"value": "1.29E-5", "module": "C2"}, {"value": "0.00146", "module": "C3"}, {"value": "7.19E-6", "module": "C4"}, {"value": "-0.0826", "module": "D"}, {"name": "referenceToUnitGroupDataSet", "value": {"shortDescription": [{"value": "m3", "lang": "en"}], "type": "unit group data set", "refObjectId": "cd950537-0a98-4044-9ba7-9f9a68d0a504", "version": "30.00.000", "uri": "../unitgroups/cd950537-0a98-4044-9ba7-9f9a68d0a504.xml"}}]}, "flowProperties": [], "typeOfFlow": "Other flow", "classification": {"classHierarchy": "Größen / Umweltliche Größen / EPD EN 15804 / LCI Indikatoren", "name": "GaBiCategories"}}, {"dataSetInternalID": 6, "referenceToFlowDataSet": {"shortDescription": [{"value": "Hazardous waste disposed (HWD)", "lang": "en"}, {"value": "Gefährlicher Abfall zur Deponie (HWD)", "lang": "de"}, {"value": "Residuos peligrosos eliminados (HWD)", "lang": "es"}], "type": "flow data set", "refObjectId": "430f9e0f-59b2-46a0-8e0d-55e0e84948fc", "version": "30.00.000", "uri": "../flows/430f9e0f-59b2-46a0-8e0d-55e0e84948fc.xml"}, "exchange direction": "OUTPUT", "meanAmount": 0.0, "other": {"anies": [{"value": "6.44E-4", "module": "A1-A3"}, {"value": "5.62E-10", "module": "A4"}, {"value": "3.14E-10", "module": "A5"}, {"value": "0.0", "module": "B1"}, {"value": "0.0", "module": "B2"}, {"value": "0.0", "module": "B3"}, {"value": "1.29E-5", "module": "B4"}, {"value": "0.0", "module": "B5"}, {"value": "0.0", "module": "B6"}, {"value": "0.0", "module": "B7"}, {"value": "0.0", "module": "C1"}, {"value": "1.4E-11", "module": "C2"}, {"value": "3.31E-9", "module": "C3"}, {"value": "6.52E-12", "module": "C4"}, {"value": "-1.51E-8", "module": "D"}, {"name": "referenceToUnitGroupDataSet", "value": {"shortDescription": [{"value": "kg", "lang": "en"}], "type": "unit group data set", "refObjectId": "ad38d542-3fe9-439d-9b95-2f5f7752acaf", "version": "30.00.000", "uri": "../unitgroups/ad38d542-3fe9-439d-9b95-2f5f7752acaf.xml"}}]}, "flowProperties": [], "typeOfFlow": "Other flow", "classification": {"classHierarchy": "Größen / Umweltliche Größen / EPD EN 15804 / LCI Indikatoren", "name": "GaBiCategories"}}, {"dataSetInternalID": 7, "referenceToFlowDataSet": {"shortDescription": [{"value": "Materials for energy recovery (MER)", "lang": "en"}, {"value": "Stoffe für die Energierückgewinnung (MER)", "lang": "de"}, {"value": "Materiales para valorización energética (recuperación de energía) (MER)", "lang": "es"}], "type": "flow data set", "refObjectId": "59a9181c-3aaf-46ee-8b13-2b3723b6e447", "version": "30.00.000", "uri": "../flows/59a9181c-3aaf-46ee-8b13-2b3723b6e447.xml"}, "exchange direction": "OUTPUT", "meanAmount": 0.0, "other": {"anies": [{"value": "0.0", "module": "A1-A3"}, {"value": "0.0", "module": "A4"}, {"value": "0.0", "module": "A5"}, {"value": "0.0", "module": "B1"}, {"value": "0.0", "module": "B2"}, {"value": "0.0", "module": "B3"}, {"value": "0.0", "module": "B4"}, {"value": "0.0", "module": "B5"}, {"value": "0.0", "module": "B6"}, {"value": "0.0", "module": "B7"}, {"value": "0.0", "module": "C1"}, {"value": "0.0", "module": "C2"}, {"value": "0.0", "module": "C3"}, {"value": "0.0", "module": "C4"}, {"value": "0.0", "module": "D"}, {"name": "referenceToUnitGroupDataSet", "value": {"shortDescription": [{"value": "kg", "lang": "en"}], "type": "unit group data set", "refObjectId": "ad38d542-3fe9-439d-9b95-2f5f7752acaf", "version": "30.00.000", "uri": "../unitgroups/ad38d542-3fe9-439d-9b95-2f5f7752acaf.xml"}}]}, "flowProperties": [], "typeOfFlow": "Other flow", "classification": {"classHierarchy": "Größen / Umweltliche Größen / EPD EN 15804 / LCI Indikatoren", "name": "GaBiCategories"}}, {"dataSetInternalID": 8, "referenceToFlowDataSet": {"shortDescription": [{"value": "Materials for recycling (MFR)", "lang": "en"}, {"value": "Stoffe zum Recycling (MFR)", "lang": "de"}, {"value": "Materiales para el reciclaje (MFR)", "lang": "es"}], "type": "flow data set", "refObjectId": "d7fe48a5-4103-49c8-9aae-b0b5dfdbd6ae", "version": "30.00.000", "uri": "../flows/d7fe48a5-4103-49c8-9aae-b0b5dfdbd6ae.xml"}, "exchange direction": "OUTPUT", "meanAmount": 0.0, "other": {"anies": [{"value": "0.46", "module": "A1-A3"}, {"value": "0.0", "module": "A4"}, {"value": "0.0", "module": "A5"}, {"value": "0.0", "module": "B1"}, {"value": "0.0", "module": "B2"}, {"value": "0.0", "module": "B3"}, {"value": "0.0651", "module": "B4"}, {"value": "0.0", "module": "B5"}, {"value": "0.0", "module": "B6"}, {"value": "0.0", "module": "B7"}, {"value": "0.0", "module": "C1"}, {"value": "0.0", "module": "C2"}, {"value": "2.8", "module": "C3"}, {"value": "0.0", "module": "C4"}, {"value": "0.0", "module": "D"}, {"name": "referenceToUnitGroupDataSet", "value": {"shortDescription": [{"value": "kg", "lang": "en"}], "type": "unit group data set", "refObjectId": "ad38d542-3fe9-439d-9b95-2f5f7752acaf", "version": "30.00.000", "uri": "../unitgroups/ad38d542-3fe9-439d-9b95-2f5f7752acaf.xml"}}]}, "flowProperties": [], "typeOfFlow": "Other flow", "classification": {"classHierarchy": "Größen / Umweltliche Größen / EPD EN 15804 / LCI Indikatoren", "name": "GaBiCategories"}}, {"dataSetInternalID": 9, "referenceToFlowDataSet": {"shortDescription": [{"value": "Non-hazardous waste disposed (NHWD)", "lang": "en"}, {"value": "Entsorgter nicht gefährlicher Abfall (NHWD)", "lang": "de"}, {"value": "Residuos no peligrosos eliminados (NHWD)", "lang": "es"}], "type": "flow data set", "refObjectId": "b29ef66b-e286-4afa-949f-62f1a7b4d7fa", "version": "30.00.000", "uri": "../flows/b29ef66b-e286-4afa-949f-62f1a7b4d7fa.xml"}, "exchange direction": "OUTPUT", "meanAmount": 0.0, "other": {"anies": [{"value": "0.42", "module": "A1-A3"}, {"value": "0.00189", "module": "A4"}, {"value": "0.0648", "module": "A5"}, {"value": "0.0", "module": "B1"}, {"value": "0.0", "module": "B2"}, {"value": "0.0", "module": "B3"}, {"value": "0.00142", "module": "B4"}, {"value": "0.0", "module": "B5"}, {"value": "0.0", "module": "B6"}, {"value": "0.0", "module": "B7"}, {"value": "0.0", "module": "C1"}, {"value": "4.7E-5", "module": "C2"}, {"value": "0.003", "module": "C3"}, {"value": "0.15", "module": "C4"}, {"value": "-0.57", "module": "D"}, {"name": "referenceToUnitGroupDataSet", "value": {"shortDescription": [{"value": "kg", "lang": "en"}], "type": "unit group data set", "refObjectId": "ad38d542-3fe9-439d-9b95-2f5f7752acaf", "version": "30.00.000", "uri": "../unitgroups/ad38d542-3fe9-439d-9b95-2f5f7752acaf.xml"}}]}, "flowProperties": [], "typeOfFlow": "Other flow", "classification": {"classHierarchy": "Größen / Umweltliche Größen / EPD EN 15804 / LCI Indikatoren", "name": "GaBiCategories"}}, {"dataSetInternalID": 10, "referenceToFlowDataSet": {"shortDescription": [{"value": "Use of non renewable secondary fuels (NRSF)", "lang": "en"}, {"value": "Nicht erneuerbare Sekundärbrennstoffe (NRSF)", "lang": "de"}, {"value": "Uso de combustibles secundarios no renovables (NRSF)", "lang": "es"}], "type": "flow data set", "refObjectId": "89def144-d39a-4287-b86f-efde453ddcb2", "version": "30.00.000", "uri": "../flows/89def144-d39a-4287-b86f-efde453ddcb2.xml"}, "exchange direction": "INPUT", "meanAmount": 0.0, "other": {"anies": [{"value": "0.0", "module": "A1-A3"}, {"value": "0.0", "module": "A4"}, {"value": "0.0", "module": "A5"}, {"value": "0.0", "module": "B1"}, {"value": "0.0", "module": "B2"}, {"value": "0.0", "module": "B3"}, {"value": "0.0", "module": "B4"}, {"value": "0.0", "module": "B5"}, {"value": "0.0", "module": "B6"}, {"value": "0.0", "module": "B7"}, {"value": "0.0", "module": "C1"}, {"value": "0.0", "module": "C2"}, {"value": "0.0", "module": "C3"}, {"value": "0.0", "module": "C4"}, {"value": "0.0", "module": "D"}, {"name": "referenceToUnitGroupDataSet", "value": {"shortDescription": [{"value": "MJ", "lang": "en"}], "type": "unit group data set", "refObjectId": "93a60a57-a3c8-11da-a746-0800200c9a66", "version": "03.00.000", "uri": "../unitgroups/93a60a57-a3c8-11da-a746-0800200c9a66.xml"}}]}, "flowProperties": [], "typeOfFlow": "Other flow", "classification": {"classHierarchy": "Größen / Umweltliche Größen / EPD EN 15804 / LCI Indikatoren", "name": "GaBiCategories"}}, {"dataSetInternalID": 11, "referenceToFlowDataSet": {"shortDescription": [{"value": "Use of non renewable primary energy (PENRE)", "lang": "en"}, {"value": "Nicht-erneuerbare Primärenergie als Energieträger (PENRE)", "lang": "de"}, {"value": "Uso de energía primaria no renovable, excluyendo los recursos de energía primaria no renovable utilizada como materia prima (PENRE)", "lang": "es"}], "type": "flow data set", "refObjectId": "ac857178-2b45-46ec-892a-a9a4332f0372", "version": "38.00.000", "uri": "../flows/ac857178-2b45-46ec-892a-a9a4332f0372.xml"}, "exchange direction": "INPUT", "meanAmount": 0.0, "other": {"anies": [{"value": "194.87", "module": "A1-A3"}, {"value": "13.3", "module": "A4"}, {"value": "2.01", "module": "A5"}, {"value": "0.0", "module": "B1"}, {"value": "0.0", "module": "B2"}, {"value": "0.0", "module": "B3"}, {"value": "2.33", "module": "B4"}, {"value": "0.0", "module": "B5"}, {"value": "0.0", "module": "B6"}, {"value": "0.0", "module": "B7"}, {"value": "0.0", "module": "C1"}, {"value": "0.33", "module": "C2"}, {"value": "3.2", "module": "C3"}, {"value": "0.0298", "module": "C4"}, {"value": "-97.1", "module": "D"}, {"name": "referenceToUnitGroupDataSet", "value": {"shortDescription": [{"value": "MJ", "lang": "en"}], "type": "unit group data set", "refObjectId": "93a60a57-a3c8-11da-a746-0800200c9a66", "version": "03.00.000", "uri": "../unitgroups/93a60a57-a3c8-11da-a746-0800200c9a66.xml"}}]}, "flowProperties": [], "typeOfFlow": "Other flow", "classification": {"classHierarchy": "Quantities", "name": "GaBiCategories"}}, {"dataSetInternalID": 12, "referenceToFlowDataSet": {"shortDescription": [{"value": "Use of non renewable primary energy resources used as raw materials (PENRM)", "lang": "en"}, {"value": "Nicht-erneuerbare Primärenergie zur stofflichen Nutzung (PENRM)", "lang": "de"}, {"value": "Uso de la energía primaria no renovable utilizada como materia prima (PENRM)", "lang": "es"}], "type": "flow data set", "refObjectId": "1421caa0-679d-4bf4-b282-0eb850ccae27", "version": "38.00.000", "uri": "../flows/1421caa0-679d-4bf4-b282-0eb850ccae27.xml"}, "exchange direction": "INPUT", "meanAmount": 0.0, "other": {"anies": [{"value": "2.09", "module": "A1-A3"}, {"value": "0.0", "module": "A4"}, {"value": "-1.4", "module": "A5"}, {"value": "0.0", "module": "B1"}, {"value": "0.0", "module": "B2"}, {"value": "0.0", "module": "B3"}, {"value": "6.91E-4", "module": "B4"}, {"value": "0.0", "module": "B5"}, {"value": "0.0", "module": "B6"}, {"value": "0.0", "module": "B7"}, {"value": "0.0", "module": "C1"}, {"value": "0.0", "module": "C2"}, {"value": "-0.66", "module": "C3"}, {"value": "0.0", "module": "C4"}, {"value": "0.0", "module": "D"}, {"name": "referenceToUnitGroupDataSet", "value": {"shortDescription": [{"value": "MJ", "lang": "en"}], "type": "unit group data set", "refObjectId": "93a60a57-a3c8-11da-a746-0800200c9a66", "version": "03.00.000", "uri": "../unitgroups/93a60a57-a3c8-11da-a746-0800200c9a66.xml"}}]}, "flowProperties": [], "typeOfFlow": "Other flow", "classification": {"classHierarchy": "Quantities", "name": "GaBiCategories"}}, {"dataSetInternalID": 13, "referenceToFlowDataSet": {"shortDescription": [{"value": "Total use of non-renewable primary energy resources (PENRT)", "lang": "en"}, {"value": "Total nicht erneuerbare Primärenergie (PENRT)", "lang": "de"}, {"value": "Uso total de la energía primaria no renovable (energía primaria y recursos de energía primaria renovable utilizada como materia prima) (PENRT)", "lang": "es"}], "type": "flow data set", "refObjectId": "06159210-646b-4c8d-8583-da9b3b95a6c1", "version": "30.00.000", "uri": "../flows/06159210-646b-4c8d-8583-da9b3b95a6c1.xml"}, "exchange direction": "INPUT", "meanAmount": 0.0, "other": {"anies": [{"value": "196.96", "module": "A1-A3"}, {"value": "13.3", "module": "A4"}, {"value": "0.62", "module": "A5"}, {"value": "0.0", "module": "B1"}, {"value": "0.0", "module": "B2"}, {"value": "0.0", "module": "B3"}, {"value": "2.33", "module": "B4"}, {"value": "0.0", "module": "B5"}, {"value": "0.0", "module": "B6"}, {"value": "0.0", "module": "B7"}, {"value": "0.0", "module": "C1"}, {"value": "0.33", "module": "C2"}, {"value": "2.54", "module": "C3"}, {"value": "0.0298", "module": "C4"}, {"value": "-97.1", "module": "D"}, {"name": "referenceToUnitGroupDataSet", "value": {"shortDescription": [{"value": "MJ", "lang": "en"}], "type": "unit group data set", "refObjectId": "93a60a57-a3c8-11da-a746-0800200c9a66", "version": "03.00.000", "uri": "../unitgroups/93a60a57-a3c8-11da-a746-0800200c9a66.xml"}}]}, "flowProperties": [], "typeOfFlow": "Other flow", "classification": {"classHierarchy": "Größen / Umweltliche Größen / EPD EN 15804 / LCI Indikatoren", "name": "GaBiCategories"}}, {"dataSetInternalID": 14, "referenceToFlowDataSet": {"shortDescription": [{"value": "Use of renewable primary energy (PERE)", "lang": "en"}, {"value": "Erneuerbare Primärenergie als Energieträger (PERE)", "lang": "de"}, {"value": "Uso de energía primaria renovable excluyendo los recursos de energía primaria renovable utilizada como materia prima (PERE)", "lang": "es"}], "type": "flow data set", "refObjectId": "20f32be5-0398-4288-9b6d-accddd195317", "version": "38.00.000", "uri": "../flows/20f32be5-0398-4288-9b6d-accddd195317.xml"}, "exchange direction": "INPUT", "meanAmount": 0.0, "other": {"anies": [{"value": "64.42", "module": "A1-A3"}, {"value": "1.01", "module": "A4"}, {"value": "20.1", "module": "A5"}, {"value": "0.0", "module": "B1"}, {"value": "0.0", "module": "B2"}, {"value": "0.0", "module": "B3"}, {"value": "1.35", "module": "B4"}, {"value": "0.0", "module": "B5"}, {"value": "0.0", "module": "B6"}, {"value": "0.0", "module": "B7"}, {"value": "0.0", "module": "C1"}, {"value": "0.0251", "module": "C2"}, {"value": "1.73", "module": "C3"}, {"value": "0.00575", "module": "C4"}, {"value": "-19.7", "module": "D"}, {"name": "referenceToUnitGroupDataSet", "value": {"shortDescription": [{"value": "MJ", "lang": "en"}], "type": "unit group data set", "refObjectId": "93a60a57-a3c8-11da-a746-0800200c9a66", "version": "03.00.000", "uri": "../unitgroups/93a60a57-a3c8-11da-a746-0800200c9a66.xml"}}]}, "flowProperties": [], "typeOfFlow": "Other flow", "classification": {"classHierarchy": "Quantities", "name": "GaBiCategories"}}, {"dataSetInternalID": 15, "referenceToFlowDataSet": {"shortDescription": [{"value": "Use of renewable primary energy resources used as raw materials (PERM)", "lang": "en"}, {"value": "Erneuerbare Primärenergie zur stofflichen Nutzung (PERM)", "lang": "de"}, {"value": "Uso de energía primaria renovable utilizada como materia prima (PERM)", "lang": "es"}], "type": "flow data set", "refObjectId": "fb3ec0de-548d-4508-aea5-00b73bf6f702", "version": "38.00.000", "uri": "../flows/fb3ec0de-548d-4508-aea5-00b73bf6f702.xml"}, "exchange direction": "INPUT", "meanAmount": 0.0, "other": {"anies": [{"value": "19.95", "module": "A1-A3"}, {"value": "0.0", "module": "A4"}, {"value": "-19.95", "module": "A5"}, {"value": "0.0", "module": "B1"}, {"value": "0.0", "module": "B2"}, {"value": "0.0", "module": "B3"}, {"value": "0.0", "module": "B4"}, {"value": "0.0", "module": "B5"}, {"value": "0.0", "module": "B6"}, {"value": "0.0", "module": "B7"}, {"value": "0.0", "module": "C1"}, {"value": "0.0", "module": "C2"}, {"value": "0.0", "module": "C3"}, {"value": "0.0", "module": "C4"}, {"value": "0.0", "module": "D"}, {"name": "referenceToUnitGroupDataSet", "value": {"shortDescription": [{"value": "MJ", "lang": "en"}], "type": "unit group data set", "refObjectId": "93a60a57-a3c8-11da-a746-0800200c9a66", "version": "03.00.000", "uri": "../unitgroups/93a60a57-a3c8-11da-a746-0800200c9a66.xml"}}]}, "flowProperties": [], "typeOfFlow": "Other flow", "classification": {"classHierarchy": "Quantities", "name": "GaBiCategories"}}, {"dataSetInternalID": 16, "referenceToFlowDataSet": {"shortDescription": [{"value": "Total use of renewable primary energy resources (PERT)", "lang": "en"}, {"value": "Total erneuerbare Primärenergie (PERT)", "lang": "de"}, {"value": "Uso total de la energía primaria renovable (energía primaria y recursos de energía primaria renovable utilizada como materia prima) (PERT)", "lang": "es"}], "type": "flow data set", "refObjectId": "53f97275-fa8a-4cdd-9024-65936002acd0", "version": "30.00.000", "uri": "../flows/53f97275-fa8a-4cdd-9024-65936002acd0.xml"}, "exchange direction": "INPUT", "meanAmount": 0.0, "other": {"anies": [{"value": "84.37", "module": "A1-A3"}, {"value": "1.01", "module": "A4"}, {"value": "0.16", "module": "A5"}, {"value": "0.0", "module": "B1"}, {"value": "0.0", "module": "B2"}, {"value": "0.0", "module": "B3"}, {"value": "1.35", "module": "B4"}, {"value": "0.0", "module": "B5"}, {"value": "0.0", "module": "B6"}, {"value": "0.0", "module": "B7"}, {"value": "0.0", "module": "C1"}, {"value": "0.0251", "module": "C2"}, {"value": "1.73", "module": "C3"}, {"value": "0.00575", "module": "C4"}, {"value": "-19.7", "module": "D"}, {"name": "referenceToUnitGroupDataSet", "value": {"shortDescription": [{"value": "MJ", "lang": "en"}], "type": "unit group data set", "refObjectId": "93a60a57-a3c8-11da-a746-0800200c9a66", "version": "03.00.000", "uri": "../unitgroups/93a60a57-a3c8-11da-a746-0800200c9a66.xml"}}]}, "flowProperties": [], "typeOfFlow": "Other flow", "classification": {"classHierarchy": "Größen / Umweltliche Größen / EPD EN 15804 / LCI Indikatoren", "name": "GaBiCategories"}}, {"dataSetInternalID": 17, "referenceToFlowDataSet": {"shortDescription": [{"value": "Use of renewable secondary fuels (RSF)", "lang": "en"}, {"value": "Erneuerbare Sekundärbrennstoffe (RSF)", "lang": "de"}, {"value": "Uso de combustibles secundarios renovables (RSF)", "lang": "es"}], "type": "flow data set", "refObjectId": "64333088-a55f-4aa2-9a31-c10b07816787", "version": "30.00.000", "uri": "../flows/64333088-a55f-4aa2-9a31-c10b07816787.xml"}, "exchange direction": "INPUT", "meanAmount": 0.0, "other": {"anies": [{"value": "0.0", "module": "A1-A3"}, {"value": "0.0", "module": "A4"}, {"value": "0.0", "module": "A5"}, {"value": "0.0", "module": "B1"}, {"value": "0.0", "module": "B2"}, {"value": "0.0", "module": "B3"}, {"value": "0.0", "module": "B4"}, {"value": "0.0", "module": "B5"}, {"value": "0.0", "module": "B6"}, {"value": "0.0", "module": "B7"}, {"value": "0.0", "module": "C1"}, {"value": "0.0", "module": "C2"}, {"value": "0.0", "module": "C3"}, {"value": "0.0", "module": "C4"}, {"value": "0.0", "module": "D"}, {"name": "referenceToUnitGroupDataSet", "value": {"shortDescription": [{"value": "MJ", "lang": "en"}], "type": "unit group data set", "refObjectId": "93a60a57-a3c8-11da-a746-0800200c9a66", "version": "03.00.000", "uri": "../unitgroups/93a60a57-a3c8-11da-a746-0800200c9a66.xml"}}]}, "flowProperties": [], "typeOfFlow": "Other flow", "classification": {"classHierarchy": "Größen / Umweltliche Größen / EPD EN 15804 / LCI Indikatoren", "name": "GaBiCategories"}}, {"dataSetInternalID": 18, "referenceToFlowDataSet": {"shortDescription": [{"value": "Radioactive waste disposed (RWD)", "lang": "en"}, {"value": "Entsorgter radioaktiver Abfall (RWD)", "lang": "de"}, {"value": "Residuos radiactivos eliminados (RWD)", "lang": "es"}], "type": "flow data set", "refObjectId": "3449546e-52ad-4b39-b809-9fb77cea8ff6", "version": "30.00.000", "uri": "../flows/3449546e-52ad-4b39-b809-9fb77cea8ff6.xml"}, "exchange direction": "OUTPUT", "meanAmount": 0.0, "other": {"anies": [{"value": "0.0126", "module": "A1-A3"}, {"value": "2.61E-5", "module": "A4"}, {"value": "3.04E-5", "module": "A5"}, {"value": "0.0", "module": "B1"}, {"value": "0.0", "module": "B2"}, {"value": "0.0", "module": "B3"}, {"value": "2.36E-4", "module": "B4"}, {"value": "0.0", "module": "B5"}, {"value": "0.0", "module": "B6"}, {"value": "0.0", "module": "B7"}, {"value": "0.0", "module": "C1"}, {"value": "6.5E-7", "module": "C2"}, {"value": "3.99E-4", "module": "C3"}, {"value": "3.16E-7", "module": "C4"}, {"value": "-0.00125", "module": "D"}, {"name": "referenceToUnitGroupDataSet", "value": {"shortDescription": [{"value": "kg", "lang": "en"}], "type": "unit group data set", "refObjectId": "ad38d542-3fe9-439d-9b95-2f5f7752acaf", "version": "30.00.000", "uri": "../unitgroups/ad38d542-3fe9-439d-9b95-2f5f7752acaf.xml"}}]}, "flowProperties": [], "typeOfFlow": "Other flow", "classification": {"classHierarchy": "Größen / Umweltliche Größen / EPD EN 15804 / LCI Indikatoren", "name": "GaBiCategories"}}, {"dataSetInternalID": 19, "referenceToFlowDataSet": {"shortDescription": [{"value": "Use of secondary material (SM)", "lang": "en"}, {"value": "Einsatz von Sekundärstoffen (SM)", "lang": "de"}, {"value": "Uso de materiales secundarios (SM)", "lang": "es"}], "type": "flow data set", "refObjectId": "c6a1f35f-2d09-4f54-8dfb-97e502e1ce92", "version": "30.00.000", "uri": "../flows/c6a1f35f-2d09-4f54-8dfb-97e502e1ce92.xml"}, "exchange direction": "INPUT", "meanAmount": 0.0, "other": {"anies": [{"value": "0.0", "module": "A1-A3"}, {"value": "0.0", "module": "A4"}, {"value": "0.0", "module": "A5"}, {"value": "0.0", "module": "B1"}, {"value": "0.0", "module": "B2"}, {"value": "0.0", "module": "B3"}, {"value": "0.0", "module": "B4"}, {"value": "0.0", "module": "B5"}, {"value": "0.0", "module": "B6"}, {"value": "0.0", "module": "B7"}, {"value": "0.0", "module": "C1"}, {"value": "0.0", "module": "C2"}, {"value": "0.0", "module": "C3"}, {"value": "0.0", "module": "C4"}, {"value": "0.0", "module": "D"}, {"name": "referenceToUnitGroupDataSet", "value": {"shortDescription": [{"value": "kg", "lang": "en"}], "type": "unit group data set", "refObjectId": "ad38d542-3fe9-439d-9b95-2f5f7752acaf", "version": "30.00.000", "uri": "../unitgroups/ad38d542-3fe9-439d-9b95-2f5f7752acaf.xml"}}]}, "flowProperties": [], "typeOfFlow": "Other flow", "classification": {"classHierarchy": "Größen / Umweltliche Größen / EPD EN 15804 / LCI Indikatoren", "name": "GaBiCategories"}}]}, "LCIAResults": {"LCIAResult": [{"referenceToLCIAMethodDataSet": {"shortDescription": [{"value": "Abiotic depletion potential - non-fossil resources (ADPE)", "lang": "en"}, {"value": "Potenzial für die Verknappung abiotischer Ressourcen – nicht fossile Ressourcen (ADPE)", "lang": "de"}], "type": "LCIA method data set", "refObjectId": "b2ad6494-c78d-11e6-9d9d-cec0c932ce01", "version": "01.00.011", "uri": "../lciamethods/b2ad6494-c78d-11e6-9d9d-cec0c932ce01.xml"}, "meanAmount": 0.0, "other": {"anies": [{"value": "5.9E-4", "module": "A1-A3"}, {"value": "6.87E-8", "module": "A4"}, {"value": "3.18E-9", "module": "A5"}, {"value": "0.0", "module": "B1"}, {"value": "0.0", "module": "B2"}, {"value": "0.0", "module": "B3"}, {"value": "7.86E-6", "module": "B4"}, {"value": "0.0", "module": "B5"}, {"value": "0.0", "module": "B6"}, {"value": "0.0", "module": "B7"}, {"value": "0.0", "module": "C1"}, {"value": "1.71E-9", "module": "C2"}, {"value": "2.58E-8", "module": "C3"}, {"value": "1.41E-10", "module": "C4"}, {"value": "-1.97E-4", "module": "D"}, {"name": "referenceToUnitGroupDataSet", "value": {"shortDescription": [{"value": "kg Sb-eq.", "lang": "en"}], "type": "unit group data set", "refObjectId": "54ccd2d9-a32a-4fc2-923d-f2c8c93e89d4", "version": "30.00.000", "uri": "../unitgroups/54ccd2d9-a32a-4fc2-923d-f2c8c93e89d4.xml"}}]}}, {"referenceToLCIAMethodDataSet": {"shortDescription": [{"value": "Abiotic depletion potential - fossil resources (ADPF)", "lang": "en"}, {"value": "Potenzial für die Verknappung abiotischer Ressourcen – fossile Brennstoffe (ADPF)", "lang": "de"}], "type": "LCIA method data set", "refObjectId": "b2ad6110-c78d-11e6-9d9d-cec0c932ce01", "version": "01.00.011", "uri": "../lciamethods/b2ad6110-c78d-11e6-9d9d-cec0c932ce01.xml"}, "meanAmount": 0.0, "other": {"anies": [{"value": "196.96", "module": "A1-A3"}, {"value": "13.3", "module": "A4"}, {"value": "0.62", "module": "A5"}, {"value": "0.0", "module": "B1"}, {"value": "0.0", "module": "B2"}, {"value": "0.0", "module": "B3"}, {"value": "2.33", "module": "B4"}, {"value": "0.0", "module": "B5"}, {"value": "0.0", "module": "B6"}, {"value": "0.0", "module": "B7"}, {"value": "0.0", "module": "C1"}, {"value": "0.33", "module": "C2"}, {"value": "2.54", "module": "C3"}, {"value": "0.0298", "module": "C4"}, {"value": "-97.1", "module": "D"}, {"name": "referenceToUnitGroupDataSet", "value": {"shortDescription": [{"value": "MJ", "lang": "en"}], "type": "unit group data set", "refObjectId": "93a60a57-a3c8-11da-a746-0800200c9a66", "version": "03.00.000", "uri": "../unitgroups/93a60a57-a3c8-11da-a746-0800200c9a66.xml"}}]}}, {"referenceToLCIAMethodDataSet": {"shortDescription": [{"value": "Acidification potential, Accumulated Exceedance (AP)", "lang": "en"}, {"value": "Versauerungspotenzial, kumulierte Überschreitung (AP)", "lang": "de"}], "type": "LCIA method data set", "refObjectId": "b5c611c6-def3-11e6-bf01-fe55135034f3", "version": "01.03.010", "uri": "../lciamethods/b5c611c6-def3-11e6-bf01-fe55135034f3.xml"}, "meanAmount": 0.0, "other": {"anies": [{"value": "0.0847", "module": "A1-A3"}, {"value": "0.00154", "module": "A4"}, {"value": "5.24E-4", "module": "A5"}, {"value": "0.0", "module": "B1"}, {"value": "0.0", "module": "B2"}, {"value": "0.0", "module": "B3"}, {"value": "9.9E-4", "module": "B4"}, {"value": "0.0", "module": "B5"}, {"value": "0.0", "module": "B6"}, {"value": "0.0", "module": "B7"}, {"value": "0.0", "module": "C1"}, {"value": "3.8E-5", "module": "C2"}, {"value": "2.86E-4", "module": "C3"}, {"value": "1.61E-5", "module": "C4"}, {"value": "-0.0376", "module": "D"}, {"name": "referenceToUnitGroupDataSet", "value": {"shortDescription": [{"value": "mol H+-eq.", "lang": "en"}], "type": "unit group data set", "refObjectId": "42e089ac-92bf-4bf2-8ca1-5fc40d18f2ed", "version": "00.01.000", "uri": "../unitgroups/42e089ac-92bf-4bf2-8ca1-5fc40d18f2ed.xml"}}]}}, {"referenceToLCIAMethodDataSet": {"shortDescription": [{"value": "Eutrophication potential - freshwater (EP-freshwater)", "lang": "en"}, {"value": "Eutrophierungspotenzial - Süßwasser (EP-freshwater)", "lang": "de"}], "type": "LCIA method data set", "refObjectId": "b53ec18f-7377-4ad3-86eb-cc3f4f276b2b", "version": "01.00.011", "uri": "../lciamethods/b53ec18f-7377-4ad3-86eb-cc3f4f276b2b.xml"}, "meanAmount": 0.0, "other": {"anies": [{"value": "4.72E-5", "module": "A1-A3"}, {"value": "2.78E-6", "module": "A4"}, {"value": "5.11E-8", "module": "A5"}, {"value": "0.0", "module": "B1"}, {"value": "0.0", "module": "B2"}, {"value": "0.0", "module": "B3"}, {"value": "9.26E-7", "module": "B4"}, {"value": "0.0", "module": "B5"}, {"value": "0.0", "module": "B6"}, {"value": "0.0", "module": "B7"}, {"value": "0.0", "module": "C1"}, {"value": "6.93E-8", "module": "C2"}, {"value": "2.66E-7", "module": "C3"}, {"value": "3.38E-9", "module": "C4"}, {"value": "-4.05E-6", "module": "D"}, {"name": "referenceToUnitGroupDataSet", "value": {"shortDescription": [{"value": "kg P-eq.", "lang": "en"}], "type": "unit group data set", "refObjectId": "0429039d-a61d-4590-ba67-aa4a20a810a1", "version": "30.00.000", "uri": "../unitgroups/0429039d-a61d-4590-ba67-aa4a20a810a1.xml"}}]}}, {"referenceToLCIAMethodDataSet": {"shortDescription": [{"value": "Eutrophication potential - marine (EP-marine)", "lang": "en"}, {"value": "Eutrophierungspotenzial - Salzwasser (EP-marine)", "lang": "de"}], "type": "LCIA method data set", "refObjectId": "b5c619fa-def3-11e6-bf01-fe55135034f3", "version": "02.00.011", "uri": "../lciamethods/b5c619fa-def3-11e6-bf01-fe55135034f3.xml"}, "meanAmount": 0.0, "other": {"anies": [{"value": "0.016", "module": "A1-A3"}, {"value": "6.31E-4", "module": "A4"}, {"value": "1.9E-4", "module": "A5"}, {"value": "0.0", "module": "B1"}, {"value": "0.0", "module": "B2"}, {"value": "0.0", "module": "B3"}, {"value": "2.36E-4", "module": "B4"}, {"value": "0.0", "module": "B5"}, {"value": "0.0", "module": "B6"}, {"value": "0.0", "module": "B7"}, {"value": "0.0", "module": "C1"}, {"value": "1.55E-5", "module": "C2"}, {"value": "6.95E-5", "module": "C3"}, {"value": "4.2E-6", "module": "C4"}, {"value": "-0.00515", "module": "D"}, {"name": "referenceToUnitGroupDataSet", "value": {"shortDescription": [{"value": "kg N-eq.", "lang": "en"}], "type": "unit group data set", "refObjectId": "d05bb823-ecdf-4686-8c40-bf1d9257859f", "version": "00.00.003", "uri": "../unitgroups/d05bb823-ecdf-4686-8c40-bf1d9257859f.xml"}}]}}, {"referenceToLCIAMethodDataSet": {"shortDescription": [{"value": "Eutrophication potential - terrestrial (EP-terrestrial)", "lang": "en"}, {"value": "Eutrophierungspotenzial - Land (EP-terrestrial)", "lang": "de"}], "type": "LCIA method data set", "refObjectId": "b5c614d2-def3-11e6-bf01-fe55135034f3", "version": "01.02.010", "uri": "../lciamethods/b5c614d2-def3-11e6-bf01-fe55135034f3.xml"}, "meanAmount": 0.0, "other": {"anies": [{"value": "0.17", "module": "A1-A3"}, {"value": "0.00659", "module": "A4"}, {"value": "0.00239", "module": "A5"}, {"value": "0.0", "module": "B1"}, {"value": "0.0", "module": "B2"}, {"value": "0.0", "module": "B3"}, {"value": "0.00247", "module": "B4"}, {"value": "0.0", "module": "B5"}, {"value": "0.0", "module": "B6"}, {"value": "0.0", "module": "B7"}, {"value": "0.0", "module": "C1"}, {"value": "1.62E-4", "module": "C2"}, {"value": "7.98E-4", "module": "C3"}, {"value": "4.58E-5", "module": "C4"}, {"value": "-0.0574", "module": "D"}, {"name": "referenceToUnitGroupDataSet", "value": {"shortDescription": [{"value": "mol N-eq.", "lang": "en"}], "type": "unit group data set", "refObjectId": "71b4d617-0ec9-4d3f-b65e-e438940c2401", "version": "00.00.003", "uri": "../unitgroups/71b4d617-0ec9-4d3f-b65e-e438940c2401.xml"}}]}}, {"referenceToLCIAMethodDataSet": {"shortDescription": [{"value": "Potential Comparative Toxic Unit for ecosystems (ETP-fw)", "lang": "en"}, {"value": "Potenzielle Toxizitätsvergleichseinheit für Ökosysteme (ETP-fw)", "lang": "de"}], "type": "LCIA method data set", "refObjectId": "05316e7a-b254-4bea-9cf0-6bf33eb5c630", "version": "01.00.003", "uri": "../lciamethods/05316e7a-b254-4bea-9cf0-6bf33eb5c630.xml"}, "meanAmount": 0.0, "other": {"anies": [{"value": "77.5", "module": "A1-A3"}, {"value": "17.2", "module": "A4"}, {"value": "0.26", "module": "A5"}, {"value": "0.0", "module": "B1"}, {"value": "0.0", "module": "B2"}, {"value": "0.0", "module": "B3"}, {"value": "1.2", "module": "B4"}, {"value": "0.0", "module": "B5"}, {"value": "0.0", "module": "B6"}, {"value": "0.0", "module": "B7"}, {"value": "0.0", "module": "C1"}, {"value": "0.43", "module": "C2"}, {"value": "0.43", "module": "C3"}, {"value": "0.023", "module": "C4"}, {"value": "-35.9", "module": "D"}, {"name": "referenceToUnitGroupDataSet", "value": {"shortDescription": [{"value": "CTUe", "lang": "en"}], "type": "unit group data set", "refObjectId": "aa959ded-f1eb-4efb-9c5c-2d60be36b3e6", "version": "00.00.003", "uri": "../unitgroups/aa959ded-f1eb-4efb-9c5c-2d60be36b3e6.xml"}}]}}, {"referenceToLCIAMethodDataSet": {"shortDescription": [{"value": "Global Warming Potential - biogenic (GWP-biogenic)", "lang": "en"}, {"value": "Globales Erwärmungspotenzial - biogen (GWP-biogenic)", "lang": "de"}], "type": "LCIA method data set", "refObjectId": "a7ea186c-9749-11ed-a8fc-0242ac120002", "version": "01.00.006", "uri": "../lciamethods/a7ea186c-9749-11ed-a8fc-0242ac120002.xml"}, "meanAmount": 0.0, "other": {"anies": [{"value": "-2.18", "module": "A1-A3"}, {"value": "0.0424", "module": "A4"}, {"value": "1.82", "module": "A5"}, {"value": "0.0", "module": "B1"}, {"value": "0.0", "module": "B2"}, {"value": "0.0", "module": "B3"}, {"value": "-0.00587", "module": "B4"}, {"value": "0.0", "module": "B5"}, {"value": "0.0", "module": "B6"}, {"value": "0.0", "module": "B7"}, {"value": "0.0", "module": "C1"}, {"value": "0.00106", "module": "C2"}, {"value": "0.00128", "module": "C3"}, {"value": "-7.35E-6", "module": "C4"}, {"value": "0.0249", "module": "D"}, {"name": "referenceToUnitGroupDataSet", "value": {"shortDescription": [{"value": "kg CO2-eq.", "lang": "en"}], "type": "unit group data set", "refObjectId": "1ebf3012-d0db-4de2-aefd-ef30cedb0be1", "version": "30.00.000", "uri": "../unitgroups/1ebf3012-d0db-4de2-aefd-ef30cedb0be1.xml"}}]}}, {"referenceToLCIAMethodDataSet": {"shortDescription": [{"value": "Global Warming Potential - fossil fuels (GWP-fossil)", "lang": "en"}, {"value": "Globales Erwärmungspotenzial - fossil (GWP-fossil)", "lang": "de"}], "type": "LCIA method data set", "refObjectId": "a7ea19c0-9749-11ed-a8fc-0242ac120002", "version": "01.00.009", "uri": "../lciamethods/a7ea19c0-9749-11ed-a8fc-0242ac120002.xml"}, "meanAmount": 0.0, "other": {"anies": [{"value": "13.74", "module": "A1-A3"}, {"value": "1.04", "module": "A4"}, {"value": "0.12", "module": "A5"}, {"value": "0.0", "module": "B1"}, {"value": "0.0", "module": "B2"}, {"value": "0.0", "module": "B3"}, {"value": "0.15", "module": "B4"}, {"value": "0.0", "module": "B5"}, {"value": "0.0", "module": "B6"}, {"value": "0.0", "module": "B7"}, {"value": "0.0", "module": "C1"}, {"value": "0.0258", "module": "C2"}, {"value": "0.17", "module": "C3"}, {"value": "0.00227", "module": "C4"}, {"value": "-7.84", "module": "D"}, {"name": "referenceToUnitGroupDataSet", "value": {"shortDescription": [{"value": "kg CO2-eq.", "lang": "en"}], "type": "unit group data set", "refObjectId": "1ebf3012-d0db-4de2-aefd-ef30cedb0be1", "version": "30.00.000", "uri": "../unitgroups/1ebf3012-d0db-4de2-aefd-ef30cedb0be1.xml"}}]}}, {"referenceToLCIAMethodDataSet": {"shortDescription": [{"value": "Global warming potential except emissions and uptake of biogenic carbon", "lang": "en"}], "type": "LCIA method data set", "refObjectId": "fb774615-0575-45de-9a89-1ded92f19770", "version": "01.00.000", "uri": "../lciamethods/fb774615-0575-45de-9a89-1ded92f19770.xml"}, "meanAmount": 0.0, "other": {"anies": [{"value": "13.799999999999999", "module": "A1-A3"}, {"value": "1.0476", "module": "A4"}, {"value": "0.1299999999999999", "module": "A5"}, {"value": "0.0", "module": "B1"}, {"value": "0.0", "module": "B2"}, {"value": "0.0", "module": "B3"}, {"value": "0.14587", "module": "B4"}, {"value": "0.0", "module": "B5"}, {"value": "0.0", "module": "B6"}, {"value": "0.0", "module": "B7"}, {"value": "0.0", "module": "C1"}, {"value": "0.02614", "module": "C2"}, {"value": "0.16872", "module": "C3"}, {"value": "0.00227735", "module": "C4"}, {"value": "-7.8549", "module": "D"}, {"name": "referenceToUnitGroupDataSet", "value": {"shortDescription": [{"value": "kg CO2-eq.", "lang": "en"}], "type": "unit group data set", "refObjectId": "1ebf3012-d0db-4de2-aefd-ef30cedb0be1", "version": "30.00.000", "uri": "../unitgroups/1ebf3012-d0db-4de2-aefd-ef30cedb0be1.xml"}}]}}, {"referenceToLCIAMethodDataSet": {"shortDescription": [{"value": "Global Warming Potential - land use and land use change (GWP-luluc)", "lang": "en"}, {"value": "Globales Erwärmungspotenzial - luluc (GWP-luluc)", "lang": "de"}], "type": "LCIA method data set", "refObjectId": "a7ea1ae2-9749-11ed-a8fc-0242ac120002", "version": "01.00.006", "uri": "../lciamethods/a7ea1ae2-9749-11ed-a8fc-0242ac120002.xml"}, "meanAmount": 0.0, "other": {"anies": [{"value": "0.0328", "module": "A1-A3"}, {"value": "0.0106", "module": "A4"}, {"value": "6.67E-5", "module": "A5"}, {"value": "0.0", "module": "B1"}, {"value": "0.0", "module": "B2"}, {"value": "0.0", "module": "B3"}, {"value": "5.77E-4", "module": "B4"}, {"value": "0.0", "module": "B5"}, {"value": "0.0", "module": "B6"}, {"value": "0.0", "module": "B7"}, {"value": "0.0", "module": "C1"}, {"value": "2.63E-4", "module": "C2"}, {"value": "4.1E-4", "module": "C3"}, {"value": "9.31E-6", "module": "C4"}, {"value": "-0.0153", "module": "D"}, {"name": "referenceToUnitGroupDataSet", "value": {"shortDescription": [{"value": "kg CO2-eq.", "lang": "en"}], "type": "unit group data set", "refObjectId": "1ebf3012-d0db-4de2-aefd-ef30cedb0be1", "version": "30.00.000", "uri": "../unitgroups/1ebf3012-d0db-4de2-aefd-ef30cedb0be1.xml"}}]}}, {"referenceToLCIAMethodDataSet": {"shortDescription": [{"value": "Global Warming Potential - total (GWP-total)", "lang": "en"}, {"value": "Globales Erwärmungspotenzial - total (GWP-total)", "lang": "de"}], "type": "LCIA method data set", "refObjectId": "a7ea142a-9749-11ed-a8fc-0242ac120002", "version": "04.00.017", "uri": "../lciamethods/a7ea142a-9749-11ed-a8fc-0242ac120002.xml"}, "meanAmount": 0.0, "other": {"anies": [{"value": "11.62", "module": "A1-A3"}, {"value": "1.09", "module": "A4"}, {"value": "1.95", "module": "A5"}, {"value": "0.0", "module": "B1"}, {"value": "0.0", "module": "B2"}, {"value": "0.0", "module": "B3"}, {"value": "0.14", "module": "B4"}, {"value": "0.0", "module": "B5"}, {"value": "0.0", "module": "B6"}, {"value": "0.0", "module": "B7"}, {"value": "0.0", "module": "C1"}, {"value": "0.0272", "module": "C2"}, {"value": "0.17", "module": "C3"}, {"value": "0.00227", "module": "C4"}, {"value": "-7.83", "module": "D"}, {"name": "referenceToUnitGroupDataSet", "value": {"shortDescription": [{"value": "kg CO2-eq.", "lang": "en"}], "type": "unit group data set", "refObjectId": "1ebf3012-d0db-4de2-aefd-ef30cedb0be1", "version": "30.00.000", "uri": "../unitgroups/1ebf3012-d0db-4de2-aefd-ef30cedb0be1.xml"}}]}}, {"referenceToLCIAMethodDataSet": {"shortDescription": [{"value": "Potential Comparative Toxic Unit for humans - cancer effects (HTP-c)", "lang": "en"}, {"value": "Potenzielle Toxizitätsvergleichseinheit für den Menschen - kanzerogene Wirkung (HTP-c)", "lang": "de"}], "type": "LCIA method data set", "refObjectId": "2299222a-bbd8-474f-9d4f-4dd1f18aea7c", "version": "01.00.004", "uri": "../lciamethods/2299222a-bbd8-474f-9d4f-4dd1f18aea7c.xml"}, "meanAmount": 0.0, "other": {"anies": [{"value": "1.97E-7", "module": "A1-A3"}, {"value": "2.32E-10", "module": "A4"}, {"value": "1.55E-11", "module": "A5"}, {"value": "0.0", "module": "B1"}, {"value": "0.0", "module": "B2"}, {"value": "0.0", "module": "B3"}, {"value": "3.69E-9", "module": "B4"}, {"value": "0.0", "module": "B5"}, {"value": "0.0", "module": "B6"}, {"value": "0.0", "module": "B7"}, {"value": "0.0", "module": "C1"}, {"value": "5.77E-12", "module": "C2"}, {"value": "4.07E-11", "module": "C3"}, {"value": "3.96E-13", "module": "C4"}, {"value": "-1.3E-8", "module": "D"}, {"name": "referenceToUnitGroupDataSet", "value": {"shortDescription": [{"value": "CTUh", "lang": "en"}], "type": "unit group data set", "refObjectId": "d4c9523e-2d7e-49fd-8469-998f547d3a70", "version": "00.00.003", "uri": "../unitgroups/d4c9523e-2d7e-49fd-8469-998f547d3a70.xml"}}]}}, {"referenceToLCIAMethodDataSet": {"shortDescription": [{"value": "Potential Comparative Toxic Unit for humans - non-cancer effects (HTP-nc)", "lang": "en"}, {"value": "Potenzielle Toxizitätsvergleichseinheit für den Menschen - nicht kanzerogene Wirkung (HTP-nc)", "lang": "de"}], "type": "LCIA method data set", "refObjectId": "7cfdcfcf-b222-4b26-888a-a55f9fbf7ac8", "version": "01.00.003", "uri": "../lciamethods/7cfdcfcf-b222-4b26-888a-a55f9fbf7ac8.xml"}, "meanAmount": 0.0, "other": {"anies": [{"value": "2.42E-7", "module": "A1-A3"}, {"value": "1.3E-8", "module": "A4"}, {"value": "3.52E-10", "module": "A5"}, {"value": "0.0", "module": "B1"}, {"value": "0.0", "module": "B2"}, {"value": "0.0", "module": "B3"}, {"value": "4.61E-9", "module": "B4"}, {"value": "0.0", "module": "B5"}, {"value": "0.0", "module": "B6"}, {"value": "0.0", "module": "B7"}, {"value": "0.0", "module": "C1"}, {"value": "3.23E-10", "module": "C2"}, {"value": "8.68E-10", "module": "C3"}, {"value": "1.48E-11", "module": "C4"}, {"value": "-2.58E-8", "module": "D"}, {"name": "referenceToUnitGroupDataSet", "value": {"shortDescription": [{"value": "CTUh", "lang": "en"}], "type": "unit group data set", "refObjectId": "d4c9523e-2d7e-49fd-8469-998f547d3a70", "version": "00.00.003", "uri": "../unitgroups/d4c9523e-2d7e-49fd-8469-998f547d3a70.xml"}}]}}, {"referenceToLCIAMethodDataSet": {"shortDescription": [{"value": "Potential Human exposure efficiency relative to U235 (IRP)", "lang": "en"}, {"value": "Potenzielle Wirkung durch Exposition des Menschen mit U235 (IRP)", "lang": "de"}], "type": "LCIA method data set", "refObjectId": "b5c632be-def3-11e6-bf01-fe55135034f3", "version": "01.00.012", "uri": "../lciamethods/b5c632be-def3-11e6-bf01-fe55135034f3.xml"}, "meanAmount": 0.0, "other": {"anies": [{"value": "1.2", "module": "A1-A3"}, {"value": "0.0037", "module": "A4"}, {"value": "0.00474", "module": "A5"}, {"value": "0.0", "module": "B1"}, {"value": "0.0", "module": "B2"}, {"value": "0.0", "module": "B3"}, {"value": "0.0215", "module": "B4"}, {"value": "0.0", "module": "B5"}, {"value": "0.0", "module": "B6"}, {"value": "0.0", "module": "B7"}, {"value": "0.0", "module": "C1"}, {"value": "9.23E-5", "module": "C2"}, {"value": "0.0659", "module": "C3"}, {"value": "3.5E-5", "module": "C4"}, {"value": "-0.21", "module": "D"}, {"name": "referenceToUnitGroupDataSet", "value": {"shortDescription": [{"value": "kgBq U235-eq.", "lang": "en"}], "type": "unit group data set", "refObjectId": "456b05bf-1415-44a9-9993-02452f554c09", "version": "00.00.003", "uri": "../unitgroups/456b05bf-1415-44a9-9993-02452f554c09.xml"}}]}}, {"referenceToLCIAMethodDataSet": {"shortDescription": [{"value": "Depletion potential of the stratospheric ozone layer (ODP)", "lang": "en"}, {"value": "Abbaupotenzial der stratosphärischen Ozonschicht (ODP)", "lang": "de"}], "type": "LCIA method data set", "refObjectId": "b5c629d6-def3-11e6-bf01-fe55135034f3", "version": "02.00.013", "uri": "../lciamethods/b5c629d6-def3-11e6-bf01-fe55135034f3.xml"}, "meanAmount": 0.0, "other": {"anies": [{"value": "6.36E-12", "module": "A1-A3"}, {"value": "1.99E-13", "module": "A4"}, {"value": "2.74E-13", "module": "A5"}, {"value": "0.0", "module": "B1"}, {"value": "0.0", "module": "B2"}, {"value": "0.0", "module": "B3"}, {"value": "-8.75E-13", "module": "B4"}, {"value": "0.0", "module": "B5"}, {"value": "0.0", "module": "B6"}, {"value": "0.0", "module": "B7"}, {"value": "0.0", "module": "C1"}, {"value": "4.97E-15", "module": "C2"}, {"value": "2.83E-12", "module": "C3"}, {"value": "6.32E-15", "module": "C4"}, {"value": "-5.34E-11", "module": "D"}, {"name": "referenceToUnitGroupDataSet", "value": {"shortDescription": [{"value": "kg CFC-11-eq.", "lang": "en"}], "type": "unit group data set", "refObjectId": "d9e957c9-7309-4474-bf3a-7777df6c4e5b", "version": "25.00.000", "uri": "../unitgroups/d9e957c9-7309-4474-bf3a-7777df6c4e5b.xml"}}]}}, {"referenceToLCIAMethodDataSet": {"shortDescription": [{"value": "Potential incidence of disease due to PM emissions (PM)", "lang": "en"}, {"value": "Potenzielles Auftreten von Krankheiten aufgrund von Feinstaubemissionen (PM)", "lang": "de"}], "type": "LCIA method data set", "refObjectId": "b5c602c6-def3-11e6-bf01-fe55135034f3", "version": "02.00.012", "uri": "../lciamethods/b5c602c6-def3-11e6-bf01-fe55135034f3.xml"}, "meanAmount": 0.0, "other": {"anies": [{"value": "1.34E-6", "module": "A1-A3"}, {"value": "1.39E-8", "module": "A4"}, {"value": "2.98E-9", "module": "A5"}, {"value": "0.0", "module": "B1"}, {"value": "0.0", "module": "B2"}, {"value": "0.0", "module": "B3"}, {"value": "1.39E-8", "module": "B4"}, {"value": "0.0", "module": "B5"}, {"value": "0.0", "module": "B6"}, {"value": "0.0", "module": "B7"}, {"value": "0.0", "module": "C1"}, {"value": "3.44E-10", "module": "C2"}, {"value": "2.32E-9", "module": "C3"}, {"value": "2.0E-10", "module": "C4"}, {"value": "-6.64E-7", "module": "D"}, {"name": "referenceToUnitGroupDataSet", "value": {"shortDescription": [{"value": "Disease incidence", "lang": "en"}], "type": "unit group data set", "refObjectId": "3883559b-648f-4afc-8ba2-0bd24f3affa3", "version": "00.00.003", "uri": "../unitgroups/3883559b-648f-4afc-8ba2-0bd24f3affa3.xml"}}]}}, {"referenceToLCIAMethodDataSet": {"shortDescription": [{"value": "Photochemical Ozone Creation Potential (POCP)", "lang": "en"}, {"value": "Bildungspotenzial für troposphärisches Ozon (POCP)", "lang": "de"}], "type": "LCIA method data set", "refObjectId": "b5c610fe-def3-11e6-bf01-fe55135034f3", "version": "02.00.015", "uri": "../lciamethods/b5c610fe-def3-11e6-bf01-fe55135034f3.xml"}, "meanAmount": 0.0, "other": {"anies": [{"value": "0.0474", "module": "A1-A3"}, {"value": "0.00137", "module": "A4"}, {"value": "5.04E-4", "module": "A5"}, {"value": "0.0", "module": "B1"}, {"value": "0.0", "module": "B2"}, {"value": "0.0", "module": "B3"}, {"value": "6.72E-4", "module": "B4"}, {"value": "0.0", "module": "B5"}, {"value": "0.0", "module": "B6"}, {"value": "0.0", "module": "B7"}, {"value": "0.0", "module": "C1"}, {"value": "3.39E-5", "module": "C2"}, {"value": "1.73E-4", "module": "C3"}, {"value": "1.26E-5", "module": "C4"}, {"value": "-0.0159", "module": "D"}, {"name": "referenceToUnitGroupDataSet", "value": {"shortDescription": [{"value": "kg NMVOC-eq.", "lang": "en"}], "type": "unit group data set", "refObjectId": "d27c25f8-fbc1-44c6-b47b-4adbae4199c6", "version": "00.00.003", "uri": "../unitgroups/d27c25f8-fbc1-44c6-b47b-4adbae4199c6.xml"}}]}}, {"referenceToLCIAMethodDataSet": {"shortDescription": [{"value": "Potential Soil quality index (SQP)", "lang": "en"}, {"value": "Potenzieller Bodenqualitätsindex (SQP)", "lang": "de"}], "type": "LCIA method data set", "refObjectId": "b2ad6890-c78d-11e6-9d9d-cec0c932ce01", "version": "01.00.011", "uri": "../lciamethods/b2ad6890-c78d-11e6-9d9d-cec0c932ce01.xml"}, "meanAmount": 0.0, "other": {"anies": [{"value": "58.22", "module": "A1-A3"}, {"value": "5.83", "module": "A4"}, {"value": "0.18", "module": "A5"}, {"value": "0.0", "module": "B1"}, {"value": "0.0", "module": "B2"}, {"value": "0.0", "module": "B3"}, {"value": "1.05", "module": "B4"}, {"value": "0.0", "module": "B5"}, {"value": "0.0", "module": "B6"}, {"value": "0.0", "module": "B7"}, {"value": "0.0", "module": "C1"}, {"value": "0.15", "module": "C2"}, {"value": "1.02", "module": "C3"}, {"value": "0.00735", "module": "C4"}, {"value": "-13.0", "module": "D"}, {"name": "referenceToUnitGroupDataSet", "value": {"shortDescription": [{"value": "dimensionless", "lang": "en"}], "type": "unit group data set", "refObjectId": "f130951c-e67f-4f7f-8dd4-665de3974e18", "version": "00.00.004", "uri": "../unitgroups/f130951c-e67f-4f7f-8dd4-665de3974e18.xml"}}]}}, {"referenceToLCIAMethodDataSet": {"shortDescription": [{"value": "Water (user) deprivation potential (WDP)", "lang": "en"}, {"value": "Wasser-Entzugspotenzial (Benutzer) (WDP)", "lang": "de"}], "type": "LCIA method data set", "refObjectId": "b2ad66ce-c78d-11e6-9d9d-cec0c932ce01", "version": "03.00.015", "uri": "../lciamethods/b2ad66ce-c78d-11e6-9d9d-cec0c932ce01.xml"}, "meanAmount": 0.0, "other": {"anies": [{"value": "8.15", "module": "A1-A3"}, {"value": "0.00515", "module": "A4"}, {"value": "0.24", "module": "A5"}, {"value": "0.0", "module": "B1"}, {"value": "0.0", "module": "B2"}, {"value": "0.0", "module": "B3"}, {"value": "0.12", "module": "B4"}, {"value": "0.0", "module": "B5"}, {"value": "0.0", "module": "B6"}, {"value": "0.0", "module": "B7"}, {"value": "0.0", "module": "C1"}, {"value": "1.28E-4", "module": "C2"}, {"value": "0.036", "module": "C3"}, {"value": "2.46E-4", "module": "C4"}, {"value": "-2.64", "module": "D"}, {"name": "referenceToUnitGroupDataSet", "value": {"shortDescription": [{"value": "m3 world eq. deprived", "lang": "en"}], "type": "unit group data set", "refObjectId": "6ae2df01-888e-46c8-b17d-49fa3869b476", "version": "00.00.003", "uri": "../unitgroups/6ae2df01-888e-46c8-b17d-49fa3869b476.xml"}}]}}]}, "otherAttributes": {"{http://www.indata.network/EPD/2019}epd-version": "1.2", "{http://www.okworx.com/ILCD/Extensions/2018/Profile}profile": "EN_15804_A2"}, "version": "1.1"}