{"processInformation": {"dataSetInformation": {"UUID": "937cf1c5-c813-4778-90e2-6f1ae84c4aa7", "name": {"baseName": [{"value": "Polyethylene piping systems for supply and disposal, industrial applications and cable protection applications", "lang": "en"}, {"value": "Polyethylen Rohrleitungssysteme für die Ver- und Entsorgung, industrielle Anwendungen und Kabelschutzanwendungen", "lang": "de"}]}, "classificationInformation": {"classification": [{"class": [{"value": "Kunststoffe", "level": 0, "classId": "6"}, {"value": "Rohre", "level": 1, "classId": "6.1"}, {"value": "Trinkwasserrohre", "level": 2, "classId": "6.1.01"}], "name": "OEKOBAU.DAT"}]}, "generalComment": [{"value": "The owner of this EPD shall be liable for the underlying information and evidence. The programme operator Kiwa-Ecobility Experts shall not be liable with respect to manufacturer data, life cycle assessment data and evidence.", "lang": "en"}, {"value": "Der Eigentümer dieser EPD haftet für die zugrunde liegenden Informationen und Nachweise. Der Programmbetreiber Kiwa-Ecobility Experts haftet nicht für die Herstellerdaten, Ökobilanzdaten und Nachweise.", "lang": "de"}], "other": {"anies": [{}, {"scenario": [{"description": [{"value": "To maintain supplier anonymity in the LCA for suppliers, they were categorized into groups. For each group, a weighted average transportation distance was calculated to accurately represent the environmental impacts associated with material transport. The weighting was based on the volume of PE supplied by each supplier, ensuring that larger suppliers had a proportionally greater influence on the overall transportation impact. Moreover, in the production process, PE offgrade material was utilized. The environmental impacts associated with the production of offgrade material were assumed to be equivalent to those of standard-grade material, as both materials undergo identical manufacturing processes. This assumption ensures that the environmental footprint of the offgrade material is aligned with the overall life cycle assessment of the primary product. For packaging of the products, the majority of the products are not individually packaged. The resulting values are derived from the calculation of average values, which are determined by considering all relevant variables such as weight, volume, or specific product characteristics. These averages are based on the annual production data. For the deconstruction of the product (module C1) a scenario was used that reflects an average deconstruction process. The weight of the raw material was set in relation to the hourly deconstruction potential of the construction machine. The value of the environmental impact was taken from a Nationale Milieudatabase (NMD) dataset stored in R< THiNK. The NMD is the Netherlands’ national environmental database, providing standardized data for assessing the environmental impact of building materials. The assumptions regarding the deconstruction potential of the construction machine were taken from a study, carried out by the NMD, listed in the references. The scenario was determined using LCA Rapportage categorie 3 data Nationale Milieudatabase - Hoofdstuk 25 Leidingwerken. In Table 12 provided data for PE pipes per meter (C1). It was assumed that the smallest diameter and lowest standard dimension ratio were used to maximize pipe length per kg of PE material, representing a worst-case scenario.", "lang": "en"}], "name": "Standard scenario", "default": true}]}, "<ns11:modules xmlns:ns11=\"http://openlca.org/epd_ilcd\" xmlns=\"http://lca.jrc.it/ILCD/Process\" xmlns:c=\"http://lca.jrc.it/ILCD/Contact\" xmlns:common=\"http://lca.jrc.it/ILCD/Common\" xmlns:epd=\"http://www.iai.kit.edu/EPD/2013\" xmlns:epd2=\"http://www.indata.network/EPD/2019\" xmlns:f=\"http://lca.jrc.it/ILCD/Flow\" xmlns:fp=\"http://lca.jrc.it/ILCD/FlowProperty\" xmlns:m=\"http://lca.jrc.it/ILCD/LCIAMethod\" xmlns:s=\"http://lca.jrc.it/ILCD/Source\" xmlns:u=\"http://lca.jrc.it/ILCD/UnitGroup\" name=\"A1\" scenario=\"Standard scenario\"/>", "<ns11:modules xmlns:ns11=\"http://openlca.org/epd_ilcd\" xmlns=\"http://lca.jrc.it/ILCD/Process\" xmlns:c=\"http://lca.jrc.it/ILCD/Contact\" xmlns:common=\"http://lca.jrc.it/ILCD/Common\" xmlns:epd=\"http://www.iai.kit.edu/EPD/2013\" xmlns:epd2=\"http://www.indata.network/EPD/2019\" xmlns:f=\"http://lca.jrc.it/ILCD/Flow\" xmlns:fp=\"http://lca.jrc.it/ILCD/FlowProperty\" xmlns:m=\"http://lca.jrc.it/ILCD/LCIAMethod\" xmlns:s=\"http://lca.jrc.it/ILCD/Source\" xmlns:u=\"http://lca.jrc.it/ILCD/UnitGroup\" name=\"A1-A3\" scenario=\"Standard scenario\"/>", "<ns11:modules xmlns:ns11=\"http://openlca.org/epd_ilcd\" xmlns=\"http://lca.jrc.it/ILCD/Process\" xmlns:c=\"http://lca.jrc.it/ILCD/Contact\" xmlns:common=\"http://lca.jrc.it/ILCD/Common\" xmlns:epd=\"http://www.iai.kit.edu/EPD/2013\" xmlns:epd2=\"http://www.indata.network/EPD/2019\" xmlns:f=\"http://lca.jrc.it/ILCD/Flow\" xmlns:fp=\"http://lca.jrc.it/ILCD/FlowProperty\" xmlns:m=\"http://lca.jrc.it/ILCD/LCIAMethod\" xmlns:s=\"http://lca.jrc.it/ILCD/Source\" xmlns:u=\"http://lca.jrc.it/ILCD/UnitGroup\" name=\"A2\" scenario=\"Standard scenario\"/>", "<ns11:modules xmlns:ns11=\"http://openlca.org/epd_ilcd\" xmlns=\"http://lca.jrc.it/ILCD/Process\" xmlns:c=\"http://lca.jrc.it/ILCD/Contact\" xmlns:common=\"http://lca.jrc.it/ILCD/Common\" xmlns:epd=\"http://www.iai.kit.edu/EPD/2013\" xmlns:epd2=\"http://www.indata.network/EPD/2019\" xmlns:f=\"http://lca.jrc.it/ILCD/Flow\" xmlns:fp=\"http://lca.jrc.it/ILCD/FlowProperty\" xmlns:m=\"http://lca.jrc.it/ILCD/LCIAMethod\" xmlns:s=\"http://lca.jrc.it/ILCD/Source\" xmlns:u=\"http://lca.jrc.it/ILCD/UnitGroup\" name=\"A3\" scenario=\"Standard scenario\"/>", "<ns11:modules xmlns:ns11=\"http://openlca.org/epd_ilcd\" xmlns=\"http://lca.jrc.it/ILCD/Process\" xmlns:c=\"http://lca.jrc.it/ILCD/Contact\" xmlns:common=\"http://lca.jrc.it/ILCD/Common\" xmlns:epd=\"http://www.iai.kit.edu/EPD/2013\" xmlns:epd2=\"http://www.indata.network/EPD/2019\" xmlns:f=\"http://lca.jrc.it/ILCD/Flow\" xmlns:fp=\"http://lca.jrc.it/ILCD/FlowProperty\" xmlns:m=\"http://lca.jrc.it/ILCD/LCIAMethod\" xmlns:s=\"http://lca.jrc.it/ILCD/Source\" xmlns:u=\"http://lca.jrc.it/ILCD/UnitGroup\" name=\"C1\" scenario=\"Standard scenario\"/>", "<ns11:modules xmlns:ns11=\"http://openlca.org/epd_ilcd\" xmlns=\"http://lca.jrc.it/ILCD/Process\" xmlns:c=\"http://lca.jrc.it/ILCD/Contact\" xmlns:common=\"http://lca.jrc.it/ILCD/Common\" xmlns:epd=\"http://www.iai.kit.edu/EPD/2013\" xmlns:epd2=\"http://www.indata.network/EPD/2019\" xmlns:f=\"http://lca.jrc.it/ILCD/Flow\" xmlns:fp=\"http://lca.jrc.it/ILCD/FlowProperty\" xmlns:m=\"http://lca.jrc.it/ILCD/LCIAMethod\" xmlns:s=\"http://lca.jrc.it/ILCD/Source\" xmlns:u=\"http://lca.jrc.it/ILCD/UnitGroup\" name=\"C2\" scenario=\"Standard scenario\"/>", "<ns11:modules xmlns:ns11=\"http://openlca.org/epd_ilcd\" xmlns=\"http://lca.jrc.it/ILCD/Process\" xmlns:c=\"http://lca.jrc.it/ILCD/Contact\" xmlns:common=\"http://lca.jrc.it/ILCD/Common\" xmlns:epd=\"http://www.iai.kit.edu/EPD/2013\" xmlns:epd2=\"http://www.indata.network/EPD/2019\" xmlns:f=\"http://lca.jrc.it/ILCD/Flow\" xmlns:fp=\"http://lca.jrc.it/ILCD/FlowProperty\" xmlns:m=\"http://lca.jrc.it/ILCD/LCIAMethod\" xmlns:s=\"http://lca.jrc.it/ILCD/Source\" xmlns:u=\"http://lca.jrc.it/ILCD/UnitGroup\" name=\"C3\" scenario=\"Standard scenario\"/>", "<ns11:modules xmlns:ns11=\"http://openlca.org/epd_ilcd\" xmlns=\"http://lca.jrc.it/ILCD/Process\" xmlns:c=\"http://lca.jrc.it/ILCD/Contact\" xmlns:common=\"http://lca.jrc.it/ILCD/Common\" xmlns:epd=\"http://www.iai.kit.edu/EPD/2013\" xmlns:epd2=\"http://www.indata.network/EPD/2019\" xmlns:f=\"http://lca.jrc.it/ILCD/Flow\" xmlns:fp=\"http://lca.jrc.it/ILCD/FlowProperty\" xmlns:m=\"http://lca.jrc.it/ILCD/LCIAMethod\" xmlns:s=\"http://lca.jrc.it/ILCD/Source\" xmlns:u=\"http://lca.jrc.it/ILCD/UnitGroup\" name=\"C4\" scenario=\"Standard scenario\"/>", "<ns11:modules xmlns:ns11=\"http://openlca.org/epd_ilcd\" xmlns=\"http://lca.jrc.it/ILCD/Process\" xmlns:c=\"http://lca.jrc.it/ILCD/Contact\" xmlns:common=\"http://lca.jrc.it/ILCD/Common\" xmlns:epd=\"http://www.iai.kit.edu/EPD/2013\" xmlns:epd2=\"http://www.indata.network/EPD/2019\" xmlns:f=\"http://lca.jrc.it/ILCD/Flow\" xmlns:fp=\"http://lca.jrc.it/ILCD/FlowProperty\" xmlns:m=\"http://lca.jrc.it/ILCD/LCIAMethod\" xmlns:s=\"http://lca.jrc.it/ILCD/Source\" xmlns:u=\"http://lca.jrc.it/ILCD/UnitGroup\" name=\"D\" scenario=\"Standard scenario\"/>", {}]}}, "quantitativeReference": {"referenceToReferenceFlow": [1], "type": "Reference flow(s)"}, "time": {"referenceYear": 2023, "dataSetValidUntil": 2029, "timeRepresentativenessDescription": [{"value": "All process-specific data was collected for the 2023 operating year. The quantities of raw materials, consumables and supplies used and the energy consumption were recorded and averaged over the entire 2023 operating year. ", "lang": "en"}, {"value": "Alle prozessspezifischen Daten wurden für das Betriebsjahr 2023 erhoben. Die eingesetzten Mengen an Roh-, Hilfs- und Betriebsstoffen sowie der Energieverbrauch wurden direkt erfasst und über das gesamte Betriebsjahr 2023 gemittelt.", "lang": "de"}], "other": {"anies": [{"name": "publicationDateOfEPD", "value": 1728864000000}]}}, "geography": {"locationOfOperationSupplyOrProduction": {"descriptionOfRestrictions": [{"value": "The reference area is Germany. \r", "lang": "en"}, {"value": "Der Referenzraum ist Deutschland.", "lang": "de"}], "location": "DE"}}, "technology": {"technologyDescriptionAndIncludedProcesses": [{"value": "The EPD is declared as average environmental performance for PE pipes that are being used for different types of supply and disposal, industrial and environmental technology as well as industrial cable conduits. The pipes are produced from polyethylen in different thicknesses, lengths and colors and are marked with colored stripes depending on the used material.\r\nMultiple product families with no significant distinction in production, raw materials, transports and packaging are included in this EPD. \r\nRCprotect®:  Pipes made of PE100-RC with colored stripes (PAS 1075 type 1) or coextruded solid wall pressure pipes with a dimensionally integrated, colored outer layer (PAS 1075 type 2) for marking the medium in accordance with the DIN EN 12201 or DIN EN 1555 standard. RCprotect® is particularly resistant to the consequences of scratches caused by the absence of sand bedding and the point loads that occur over a longer period of time. \r\nGEROthen®: Either single-layer extruded black pipes with medium-specific color stripe marking or double-layer co-extruded solid-wall pipes in material class PE100 in accordance with DIN EN 12201 or DIN EN 1555.  \r\nGEROblanco®: Sewer pipe systems in accordance with DIN EN 12201. They are a fully weldable pipe system made of PE100 or PE100-RC. It is so flexible that deformations can be absorbed by the system without causing cracks and, thus, leaks. Welding using electrofusion couplings guarantees a permanently tight and longitudinally and transversely force-locked connection between the pipes.  \r\nLHT INDUSTRY®: Pressure pipes made of PE-RT (Raised Temperature) in accordance with DIN EN ISO 15494 for industrial and environmental applications. Extended application potential and new areas of use at operating temperatures from -40°C to +95°C. \r\nGEROtec MINING®: Abrasion-resistant pressure pipe made of PE100 or PE100-RC in accordance with DIN EN 12201 for mining and open-cast mining. The inner protective layer made of TPE guarantees long-term resistance to abrasive wear during the transportation of materials containing solids. Available as 2-layer (GEROtec MINING I) or 3-layer (GEROtec MINING II) system pipe.  \r\nGEROtec FIRE-MAIN®:  Pipe system in accordance with DIN EN ISO 15494 for underground, public and industrial extinguishing water networks made of PE100-RC material with colored longitudinal stripes evenly distributed around the pipe circumference or co-extruded colored outer layer. \r\nGEROtec ANERGIE®: Solid-wall pressure pipes made of resistant PE100-RC in accordance with DIN EN ISO 15494 with colored longitudinal stripes distributed around the pipe circumference. Used for highly efficient cooling and heating of buildings with cold district heating. Optimized as a supply and return pipe for heat absorption and dissipation.  \r\nLHT E-Power cable conduit®:  Protective pipes made of PE-RT (Raised Temperature) in accordance with DIN 16874, DIN 16876 and DIN 16842 with colored longitudinal stripes evenly distributed around the pipe circumference or coextruded colored outer layer. Used for underground cabling of high and extra-high voltage lines up to 525 kV and a continuous service temperature of over 70°C. \r\nEMDS®:  Cable protection conduits made of the material PE-HD+ (PE according to DIN 16874), PE100 or PE100-RC according to DIN 16874, DIN 16876 and DIN 16842 with or without colored longitudinal stripes evenly distributed around the circumference of the conduit or a colored outer layer. GEROtherm ground collector pipe®: Pressure pipe made of PE100-RC material to DIN EN ISO 15494 with green longitudinal stripes evenly distributed around the circumference of the pipe or co-extruded green outer layer. Used for underground installation and brine distribution up to 40°C.\r\n\r\nThe different types / grades of PE are being transported to the factory, where they will be transported internally via forklifts to the extrusion machine. There, the extrusion process is carried out, where the PE mix is heated and then pushed through a die with adjustable thickness. Through the sheer pressure the material is put through the die with, it gains the desired form and thickness for the needed pipe. The pipe is then cooled with water so it retains its form. It is then signed, checked for quality and lastly cut into the desired length. Then the product is packaged and prepared for transport.\r\n", "lang": "en"}, {"value": "Die Umweltproduktdeklaration (EPD) wird als durchschnittliche Umweltleistung für PE Rohre angegeben, die für verschiedene Arten der Ver- und Entsorgung, Industrie- und Umwelttechnik sowie für industrielle Kabelkanäle verwendet werden. Die Rohre werden aus Polyethylen in verschiedenen Stärken, Längen und Farben hergestellt und je nach verwendetem Material mit farbigen Streifen gekennzeichnet. \r\nDiese Umweltproduktdeklaration umfasst mehrere Produktfamilien ohne wesentliche Unterschiede in der Produktion, den Rohstoffen, den Transporten und der Verpackung. RCprotect®: Rohre aus PE100-RC mit Farbstreifen (PAS 1075 Typ 1) oder coextrudierte Vollwand-Druckrohre mit maßlich integrierter farbiger Außenschicht (PAS 1075 Typ 2) zur Kennzeichnung des Mediums nach DIN EN 12201 bzw. DIN EN 1555. \r\nRCprotect® ist besonders widerstandsfähig gegen die Folgen von Kratzern, die durch das Fehlen einer Sandbettung entstehen, und gegen Punktlasten, die über einen längeren Zeitraum auftreten. GEROthen®: Entweder einschichtig extrudierte schwarze Rohre mit medienspezifischer Farbstreifenmarkierung oder zweischichtig coextrudierte Vollwandrohre der Materialklasse PE100 nach DIN EN 12201 oder DIN EN 1555. \r\nGEROblanco®: Kanalrohrsysteme nach DIN EN 12201. Es handelt sich um ein vollverschweißbares Rohrsystem aus PE100 oder PE100-RC. Es ist so flexibel, dass Verformungen vom System aufgenommen werden können, ohne dass es zu Rissen und damit zu Undichtigkeiten kommt. Die Verschweißung mittels Elektroschweißmuffen garantiert eine dauerhaft dichte und längs- und querkraftschlüssige Verbindung der Rohre. \r\nLHT INDUSTRY®: Druckrohre aus PE-RT (Raised Temperature) nach DIN EN ISO 15494 für Industrie- und Umweltanwendungen. Erweitertes Anwendungspotenzial und neue Einsatzbereiche bei Betriebstemperaturen von -40 °C bis +95 °C. \r\nGEROtec MINING®: Abriebfestes Druckrohr aus PE100 oder PE100-RC nach DIN EN 12201 für den Berg- und Tagebau. Die Innenschutzschicht aus TPE garantiert eine dauerhafte Beständigkeit gegen abrasiven Verschleiß beim Transport feststoffhaltiger Materialien. Als 2-Schicht- (GEROtec MINING I) oder 3-Schicht-Systemrohr (GEROtec MINING II) erhältlich.\r\nGEROtec FIRE-MAIN®: Rohrsystem nach DIN EN ISO 15494 für erdverlegte, öffentliche und industrielle Löschwasserleitungen aus PE100-RC-Material mit gleichmäßig über den Rohrumfang verteilten farbigen Längsstreifen oder coextrudierter farbiger Außenschicht. \r\nGEROtec ANERGIE®: Vollwandige Druckrohre aus widerstandsfähigem PE100-RC nach DIN EN ISO 15494 mit um den Rohrumfang verteilten farbigen Längsstreifen. Einsatz zur hocheffizienten Kühlung und Beheizung von Gebäuden mit kalter Fernwärme. Optimiert als Vor- und Rücklaufleitung zur Wärmeaufnahme und -abgabe. \r\nLHT E-Power cable conduit®: Schutzrohre aus PE-RT (Raised Temperature) nach DIN 16874, DIN 16876 und DIN 16842 mit gleichmäßig über den Rohrumfang verteilten farbigen Längsstreifen oder koextrudierter farbiger Außenschicht. Einsatz für die Erdverkabelung von Hoch- und Höchstspannungsleitungen bis 525 kV und einer Dauergebrauchstemperatur von über 70 °C. \r\nEMDS®: Kabelschutzrohre aus dem Werkstoff PE-HD+ (PE nach DIN 16874), PE100 oder PE100-RC nach DIN 16874, DIN 16876 und DIN 16842 mit oder ohne gleichmäßig über den Umfang verteilten farbigen Längsstreifen oder farbiger Außenschicht. \r\nGEROtherm Erdkollektorrohr®: Druckrohr aus PE100-RC-Material nach DIN EN ISO 15494 mit gleichmäßig über den Rohrumfang verteilten grünen Längsstreifen oder coextrudierter grüner Außenschicht. Verwendung für die Erdverlegung und Soleverteilung bis 40 °C.\r\nDie verschiedenen Arten/Klassen von PE werden zur Fabrik transportiert, wo sie intern mit Gabelstaplern zur Extrusionsmaschine transportiert werden. Dort wird der Extrusionsprozess durchgeführt, bei dem die PE-Mischung erhitzt und dann durch eine Düse mit einstellbarer Dicke gepresst wird. Durch den bloßen Druck, mit dem das Material durch die Düse gepresst wird, erhält es die gewünschte Form und Dicke für das benötigte Rohr. Das Rohr wird dann mit Wasser gekühlt, damit es seine Form behält. Anschließend wird es signiert, auf Qualität geprüft und schließlich auf die gewünschte Länge zugeschnitten. Dann wird das Produkt verpackt und für den Transport vorbereitet.\r\nDie in dieser EPD enthaltenen PE-Rohre können für eine Vielzahl von Funktionen eingesetzt werden. Je nach Rohr werden sie für die Ver- und Entsorgung, die Industrie und Umwelttechnik sowie als industrielle Kabelschutzrohre verwendet. \r\n", "lang": "de"}], "technologicalApplicability": [{"value": "The PE-pipes included in this EPD can be used for a wide array of functions. Depending on the specific pipe, they are being used for supply and disposal, industrial and environmental technology as well as industrial cable conduits. ", "lang": "en"}, {"value": "Die in dieser EPD enthaltenen PE-Rohre können für eine Vielzahl von Funktionen eingesetzt werden. Je nach Rohr werden sie für die Ver- und Entsorgung, die Industrie und Umwelttechnik sowie als industrielle Kabelschutzrohre verwendet. ", "lang": "de"}], "referenceToTechnologyFlowDiagrammOrPicture": [{"shortDescription": [{"value": "Flowchart Gerodur, Polyethylene piping systems for supply and disposal, industrial applications and cable protection applications", "lang": "en"}], "type": "source data set", "refObjectId": "660af336-4655-4bdf-bc39-60d0d934f9a0", "version": "00.00.001"}]}}, "modellingAndValidation": {"LCIMethodAndAllocation": {"typeOfDataSet": "EPD", "other": {"anies": [{"name": "subType", "value": "average dataset"}]}}, "dataSourcesTreatmentAndRepresentativeness": {"referenceToDataSource": [{"shortDescription": [{"value": "ecoinvent 3.6 database", "lang": "en"}], "type": "source data set", "refObjectId": "766b9973-5ee8-48a2-8098-72c8e20b369f", "version": "00.00.001"}, {"shortDescription": [{"value": "ecoinvent database (general)", "lang": "en"}], "type": "source data set", "refObjectId": "b497a91f-e14b-4b69-8f28-f50eb1576766", "version": "00.03.002"}], "useAdviceForDataSet": [{"value": "The PE-pipes included in this EPD can be used for a wide array of functions. Depending on the specific pipe, they are being used for supply and disposal, industrial and environmental technology as well as industrial cable conduits. ", "lang": "en"}, {"value": "Die in dieser EPD enthaltenen PE-Rohre können für eine Vielzahl von Funktionen eingesetzt werden. Je nach Rohr werden sie für die Ver- und Entsorgung, die Industrie und Umwelttechnik sowie als industrielle Kabelschutzrohre verwendet. ", "lang": "de"}], "other": {"anies": [{"name": "referenceToOriginalEPD", "value": {"shortDescription": {"value": "Polyethylen Rohrleitungssysteme für die Ver- und Entsorgung, industrielle Anwendungen und Kabelschutzanwendungen (Gerodur MPM Kunststoffverarbeitung) EPD", "defaultValue": "Polyethylen Rohrleitungssysteme für die Ver- und Entsorgung, industrielle Anwendungen und Kabelschutzanwendungen (Gerodur MPM Kunststoffverarbeitung) EPD", "lstrings": [{"lang": "de", "value": "Polyethylen Rohrleitungssysteme für die Ver- und Entsorgung, industrielle Anwendungen und Kabelschutzanwendungen (Gerodur MPM Kunststoffverarbeitung) EPD"}, {"lang": "en", "value": "Polyethylene piping systems for supply and disposal, industrial applications and cable protection applications (Gerodur MPM Kunststoffverarbeitung) EPD"}]}, "version": {"version": 2, "majorVersion": 0, "minorVersion": 0, "subMinorVersion": 2, "zero": false, "versionString": "00.00.002"}, "type": "source data set", "uuid": {"uuid": "e97a3113-b1d6-403c-af91-94f2d15540ce"}, "refObjectId": "e97a3113-b1d6-403c-af91-94f2d15540ce", "versionAsString": "00.00.002", "resourceURLs": ["https://oekobaudat.de/OEKOBAU.DAT/resource/sources/e97a3113-b1d6-403c-af91-94f2d15540ce/EPD-Kiwa-EE-184625-DE.pdf?version=00.00.002", "https://oekobaudat.de/OEKOBAU.DAT/resource/sources/e97a3113-b1d6-403c-af91-94f2d15540ce/EPD-Kiwa-EE-179667-EN.pdf?version=00.00.002"]}}]}}, "validation": {"review": [{"reviewDetails": [{"value": "The independent verification is in accordance with the ISO 14025:2011", "lang": "en"}, {"value": "Die unabhängige Verifizierung erfolgt gemäß der ISO 14025:2011.", "lang": "de"}], "referenceToNameOfReviewerAndInstitution": [{"shortDescription": [{"value": "Lucas Pedro Berman, Senda", "lang": "en"}], "type": "contact data set", "refObjectId": "2294137c-5a52-4a75-965f-770e74b24b10", "version": "00.00.002"}], "type": "Independent external review"}]}, "complianceDeclarations": {"compliance": [{"referenceToComplianceSystem": {"shortDescription": [{"value": "EN 15804+A2 (EF 3.1)", "lang": "de"}, {"value": "EN 15804+A2 (EF 3.1)", "lang": "en"}], "type": "source data set", "refObjectId": "d4aa3ec7-b1d7-4a4a-a6cb-37af88dcc902", "version": "00.01.000"}}, {"referenceToComplianceSystem": {"shortDescription": [{"value": "ISO 14025", "lang": "en"}], "type": "source data set", "refObjectId": "4f2eb655-6e44-4874-a95a-e28f5442cd4d", "version": "00.00.001"}}]}}, "administrativeInformation": {"commissionerAndGoal": {"referenceToCommissioner": [{"shortDescription": [{"value": "Gerodur MPM Kunststoffverarbeitung GmbH & Co. KG", "lang": "en"}], "type": "contact data set", "refObjectId": "daf67ca3-4ec5-400d-9586-f796c3d55f59", "version": "00.00.001"}]}, "dataGenerator": {"referenceToPersonOrEntityGeneratingTheDataSet": [{"shortDescription": [{"value": "Kiwa GmbH (Berlin)", "lang": "en"}], "type": "contact data set", "refObjectId": "3ea4a87a-3f88-4633-b7e7-1bbdd272be43", "version": "00.00.002"}]}, "dataEntryBy": {"timeStamp": 1738148765700, "referenceToDataSetFormat": [{"shortDescription": [{"value": "EPD Data Format Extensions v1.2", "lang": "en"}, {"value": "EPD-Datenformaterweiterungen v1.2", "lang": "de"}], "type": "source data set", "refObjectId": "a29449fd-aa2f-4de8-b5d7-4b06b43c6fde", "version": "00.01.000"}, {"shortDescription": [{"value": "ILCD format", "lang": "en"}], "type": "source data set", "refObjectId": "a97a0155-0234-4b87-b4ce-a45da52f2a40", "version": "01.00.000", "uri": "http://lca.jrc.ec.europa.eu/lcainfohub/sample_data/ilcd/sources/ILCD_Format_a97a0155-0234-4b87-b4ce-a45da52f2a40_01.00.000.xml"}], "referenceToPersonOrEntityEnteringTheData": {"shortDescription": [{"value": "Kiwa GmbH (Berlin)", "lang": "en"}], "type": "contact data set", "refObjectId": "3ea4a87a-3f88-4633-b7e7-1bbdd272be43", "version": "00.00.002"}}, "publicationAndOwnership": {"dataSetVersion": "00.00.007", "referenceToRegistrationAuthority": {"shortDescription": [{"value": "Kiwa-Ecobility Experts, Kiwa GmbH (Berlin)", "lang": "en"}], "type": "contact data set", "refObjectId": "eb52a9a8-9d0f-40ce-a5c9-7b78f5615e5a", "version": "00.00.002"}, "registrationNumber": "EPD-Kiwa-EE-179667-EN, EPD-Kiwa-EE-184625-DE", "referenceToOwnershipOfDataSet": {"shortDescription": [{"value": "Gerodur MPM Kunststoffverarbeitung GmbH & Co. KG", "lang": "en"}], "type": "contact data set", "refObjectId": "daf67ca3-4ec5-400d-9586-f796c3d55f59", "version": "00.00.001"}, "copyright": true, "licenseType": "Free of charge for all users and uses", "accessRestrictions": [{"value": "None.", "lang": "en"}, {"value": "Keine.", "lang": "de"}], "other": {"anies": [{"name": "referenceToPublisher", "value": {"shortDescription": [{"value": "Kiwa-Ecobility Experts, Kiwa GmbH (Berlin)", "lang": "en"}], "type": "contact data set", "refObjectId": "eb52a9a8-9d0f-40ce-a5c9-7b78f5615e5a", "version": "00.00.002"}}]}}}, "exchanges": {"exchange": [{"dataSetInternalID": 1, "referenceToFlowDataSet": {"shortDescription": [{"value": "Polyethylene piping systems for supply and disposal, industrial applications and cable protection applications", "lang": "en"}, {"value": "Polyethylen Rohrleitungssysteme für die Ver- und Entsorgung, industrielle Anwendungen und Kabelschutzanwendungen", "lang": "de"}], "type": "flow data set", "refObjectId": "e9e8ef42-da42-4794-99d1-f097d9c15686", "version": "00.00.002"}, "meanAmount": 1.0, "resultingAmount": 1.0, "referenceFlow": true, "resultingflowAmount": 1.0, "flowProperties": [{"name": [{"lang": "en", "value": "Mass"}, {"lang": "de", "value": "Masse"}], "uuid": "93a60a56-a3c8-11da-a746-0800200b9a66", "referenceFlowProperty": true, "meanValue": 1.0, "referenceUnit": "kg", "unitGroupUUID": "ad38d542-3fe9-439d-9b95-2f5f7752acaf"}], "materialProperties": [{"name": "gross density", "value": "950.0", "unit": "kg/m^3", "unitDescription": "kilograms per cubic metre"}], "typeOfFlow": "Product flow", "classification": {"classHierarchy": "Kunststoffe / Rohre / Trinkwasserrohre", "name": "OEKOBAU.DAT"}}, {"dataSetInternalID": 2, "referenceToFlowDataSet": {"shortDescription": [{"value": "Components for re-use (CRU)", "lang": "en"}, {"value": "Komponenten für die Wiederverwendung (CRU)", "lang": "de"}, {"value": "Componentes para su reutilización (CRU)", "lang": "es"}], "type": "flow data set", "refObjectId": "a2b32f97-3fc7-4af2-b209-525bc6426f33", "version": "30.00.000", "uri": "../flows/a2b32f97-3fc7-4af2-b209-525bc6426f33.xml"}, "exchange direction": "OUTPUT", "meanAmount": 0.0, "other": {"anies": [{"value": "0.0", "module": "A1", "scenario": "Standard scenario"}, {"value": "0.0", "module": "A2", "scenario": "Standard scenario"}, {"value": "0.0", "module": "A3", "scenario": "Standard scenario"}, {"value": "0.0", "module": "A1-A3", "scenario": "Standard scenario"}, {"value": "0.0", "module": "C1", "scenario": "Standard scenario"}, {"value": "0.0", "module": "C2", "scenario": "Standard scenario"}, {"value": "0.0", "module": "C3", "scenario": "Standard scenario"}, {"value": "0.0", "module": "C4", "scenario": "Standard scenario"}, {"value": "0.0", "module": "D", "scenario": "Standard scenario"}, {"name": "referenceToUnitGroupDataSet", "value": {"shortDescription": [{"value": "kg", "lang": "en"}], "type": "unit group data set", "refObjectId": "ad38d542-3fe9-439d-9b95-2f5f7752acaf", "version": "30.00.000", "uri": "../unitgroups/ad38d542-3fe9-439d-9b95-2f5f7752acaf.xml"}}]}, "flowProperties": [], "typeOfFlow": "Other flow", "classification": {"classHierarchy": "Größen / Umweltliche Größen / EPD EN 15804 / LCI Indikatoren", "name": "GaBiCategories"}}, {"dataSetInternalID": 3, "referenceToFlowDataSet": {"shortDescription": [{"value": "Exported electrical energy (EEE)", "lang": "en"}, {"value": "Exportierte elektrische Energie (EEE)", "lang": "de"}, {"value": "Energía exportada electrica (EEE)", "lang": "es"}], "type": "flow data set", "refObjectId": "4da0c987-2b76-40d6-9e9e-82a017aaaf29", "version": "30.00.000", "uri": "../flows/4da0c987-2b76-40d6-9e9e-82a017aaaf29.xml"}, "exchange direction": "OUTPUT", "meanAmount": 0.0, "other": {"anies": [{"value": "0.0", "module": "A1", "scenario": "Standard scenario"}, {"value": "0.0", "module": "A2", "scenario": "Standard scenario"}, {"value": "-0.0607143059982", "module": "A3", "scenario": "Standard scenario"}, {"value": "-0.0607143059982", "module": "A1-A3", "scenario": "Standard scenario"}, {"value": "0.0", "module": "C1", "scenario": "Standard scenario"}, {"value": "0.0", "module": "C2", "scenario": "Standard scenario"}, {"value": "0.0", "module": "C3", "scenario": "Standard scenario"}, {"value": "0.0", "module": "C4", "scenario": "Standard scenario"}, {"value": "-3.57142976459999", "module": "D", "scenario": "Standard scenario"}, {"name": "referenceToUnitGroupDataSet", "value": {"shortDescription": [{"value": "MJ", "lang": "en"}], "type": "unit group data set", "refObjectId": "93a60a57-a3c8-11da-a746-0800200c9a66", "version": "03.00.000", "uri": "../unitgroups/93a60a57-a3c8-11da-a746-0800200c9a66.xml"}}]}, "flowProperties": [], "typeOfFlow": "Other flow", "classification": {"classHierarchy": "Größen / Umweltliche Größen / EPD EN 15804 / LCI Indikatoren", "name": "GaBiCategories"}}, {"dataSetInternalID": 4, "referenceToFlowDataSet": {"shortDescription": [{"value": "Exported thermal energy (EET)", "lang": "en"}, {"value": "Exportierte thermische Energie (EET)", "lang": "de"}, {"value": "Energía exportada termal (EET)", "lang": "es"}], "type": "flow data set", "refObjectId": "98daf38a-7a79-46d3-9a37-2b7bd0955810", "version": "30.00.000", "uri": "../flows/98daf38a-7a79-46d3-9a37-2b7bd0955810.xml"}, "exchange direction": "OUTPUT", "meanAmount": 0.0, "other": {"anies": [{"value": "0.0", "module": "A1", "scenario": "Standard scenario"}, {"value": "0.0", "module": "A2", "scenario": "Standard scenario"}, {"value": "-0.1045635269969", "module": "A3", "scenario": "Standard scenario"}, {"value": "-0.1045635269969", "module": "A1-A3", "scenario": "Standard scenario"}, {"value": "0.0", "module": "C1", "scenario": "Standard scenario"}, {"value": "0.0", "module": "C2", "scenario": "Standard scenario"}, {"value": "0.0", "module": "C3", "scenario": "Standard scenario"}, {"value": "0.0", "module": "C4", "scenario": "Standard scenario"}, {"value": "-6.1507957057", "module": "D", "scenario": "Standard scenario"}, {"name": "referenceToUnitGroupDataSet", "value": {"shortDescription": [{"value": "MJ", "lang": "en"}], "type": "unit group data set", "refObjectId": "93a60a57-a3c8-11da-a746-0800200c9a66", "version": "03.00.000", "uri": "../unitgroups/93a60a57-a3c8-11da-a746-0800200c9a66.xml"}}]}, "flowProperties": [], "typeOfFlow": "Other flow", "classification": {"classHierarchy": "Größen / Umweltliche Größen / EPD EN 15804 / LCI Indikatoren", "name": "GaBiCategories"}}, {"dataSetInternalID": 5, "referenceToFlowDataSet": {"shortDescription": [{"value": "Use of net fresh water (FW)", "lang": "en"}, {"value": "Einsatz von Süßwasserressourcen (FW)", "lang": "de"}, {"value": "Uso neto de recursos de agua dulce (FW)", "lang": "es"}], "type": "flow data set", "refObjectId": "3cf952c8-f3a4-461d-8c96-96456ca62246", "version": "30.00.000", "uri": "../flows/3cf952c8-f3a4-461d-8c96-96456ca62246.xml"}, "exchange direction": "INPUT", "meanAmount": 0.0, "other": {"anies": [{"value": "0.023394688209692", "module": "A1", "scenario": "Standard scenario"}, {"value": "1.771410743783E-4", "module": "A2", "scenario": "Standard scenario"}, {"value": "0.00237845178949", "module": "A3", "scenario": "Standard scenario"}, {"value": "0.025950281073560302", "module": "A1-A3", "scenario": "Standard scenario"}, {"value": "2.533460971679E-4", "module": "C1", "scenario": "Standard scenario"}, {"value": "3.47103991682E-5", "module": "C2", "scenario": "Standard scenario"}, {"value": "0.00339785", "module": "C3", "scenario": "Standard scenario"}, {"value": "2.62E-5", "module": "C4", "scenario": "Standard scenario"}, {"value": "-0.0011199682017671", "module": "D", "scenario": "Standard scenario"}, {"name": "referenceToUnitGroupDataSet", "value": {"shortDescription": [{"value": "m3", "lang": "en"}], "type": "unit group data set", "refObjectId": "cd950537-0a98-4044-9ba7-9f9a68d0a504", "version": "30.00.000", "uri": "../unitgroups/cd950537-0a98-4044-9ba7-9f9a68d0a504.xml"}}]}, "flowProperties": [], "typeOfFlow": "Other flow", "classification": {"classHierarchy": "Größen / Umweltliche Größen / EPD EN 15804 / LCI Indikatoren", "name": "GaBiCategories"}}, {"dataSetInternalID": 6, "referenceToFlowDataSet": {"shortDescription": [{"value": "Hazardous waste disposed (HWD)", "lang": "en"}, {"value": "Gefährlicher Abfall zur Deponie (HWD)", "lang": "de"}, {"value": "Residuos peligrosos eliminados (HWD)", "lang": "es"}], "type": "flow data set", "refObjectId": "430f9e0f-59b2-46a0-8e0d-55e0e84948fc", "version": "30.00.000", "uri": "../flows/430f9e0f-59b2-46a0-8e0d-55e0e84948fc.xml"}, "exchange direction": "OUTPUT", "meanAmount": 0.0, "other": {"anies": [{"value": "1.188609802E-5", "module": "A1", "scenario": "Standard scenario"}, {"value": "3.6768971684E-6", "module": "A2", "scenario": "Standard scenario"}, {"value": "1.8908740138E-6", "module": "A3", "scenario": "Standard scenario"}, {"value": "1.7453869202200003E-5", "module": "A1-A3", "scenario": "Standard scenario"}, {"value": "1.34045080875E-5", "module": "C1", "scenario": "Standard scenario"}, {"value": "7.220914355E-7", "module": "C2", "scenario": "Standard scenario"}, {"value": "3.3215E-6", "module": "C3", "scenario": "Standard scenario"}, {"value": "3.81E-8", "module": "C4", "scenario": "Standard scenario"}, {"value": "-1.84676823405E-5", "module": "D", "scenario": "Standard scenario"}, {"name": "referenceToUnitGroupDataSet", "value": {"shortDescription": [{"value": "kg", "lang": "en"}], "type": "unit group data set", "refObjectId": "ad38d542-3fe9-439d-9b95-2f5f7752acaf", "version": "30.00.000", "uri": "../unitgroups/ad38d542-3fe9-439d-9b95-2f5f7752acaf.xml"}}]}, "flowProperties": [], "typeOfFlow": "Other flow", "classification": {"classHierarchy": "Größen / Umweltliche Größen / EPD EN 15804 / LCI Indikatoren", "name": "GaBiCategories"}}, {"dataSetInternalID": 7, "referenceToFlowDataSet": {"shortDescription": [{"value": "Materials for energy recovery (MER)", "lang": "en"}, {"value": "Stoffe für die Energierückgewinnung (MER)", "lang": "de"}, {"value": "Materiales para valorización energética (recuperación de energía) (MER)", "lang": "es"}], "type": "flow data set", "refObjectId": "59a9181c-3aaf-46ee-8b13-2b3723b6e447", "version": "30.00.000", "uri": "../flows/59a9181c-3aaf-46ee-8b13-2b3723b6e447.xml"}, "exchange direction": "OUTPUT", "meanAmount": 0.0, "other": {"anies": [{"value": "0.0", "module": "A1", "scenario": "Standard scenario"}, {"value": "0.0", "module": "A2", "scenario": "Standard scenario"}, {"value": "0.0", "module": "A3", "scenario": "Standard scenario"}, {"value": "0.0", "module": "A1-A3", "scenario": "Standard scenario"}, {"value": "0.0", "module": "C1", "scenario": "Standard scenario"}, {"value": "0.0", "module": "C2", "scenario": "Standard scenario"}, {"value": "0.0", "module": "C3", "scenario": "Standard scenario"}, {"value": "0.0", "module": "C4", "scenario": "Standard scenario"}, {"value": "0.0", "module": "D", "scenario": "Standard scenario"}, {"name": "referenceToUnitGroupDataSet", "value": {"shortDescription": [{"value": "kg", "lang": "en"}], "type": "unit group data set", "refObjectId": "ad38d542-3fe9-439d-9b95-2f5f7752acaf", "version": "30.00.000", "uri": "../unitgroups/ad38d542-3fe9-439d-9b95-2f5f7752acaf.xml"}}]}, "flowProperties": [], "typeOfFlow": "Other flow", "classification": {"classHierarchy": "Größen / Umweltliche Größen / EPD EN 15804 / LCI Indikatoren", "name": "GaBiCategories"}}, {"dataSetInternalID": 8, "referenceToFlowDataSet": {"shortDescription": [{"value": "Materials for recycling (MFR)", "lang": "en"}, {"value": "Stoffe zum Recycling (MFR)", "lang": "de"}, {"value": "Materiales para el reciclaje (MFR)", "lang": "es"}], "type": "flow data set", "refObjectId": "d7fe48a5-4103-49c8-9aae-b0b5dfdbd6ae", "version": "30.00.000", "uri": "../flows/d7fe48a5-4103-49c8-9aae-b0b5dfdbd6ae.xml"}, "exchange direction": "OUTPUT", "meanAmount": 0.0, "other": {"anies": [{"value": "0.0", "module": "A1", "scenario": "Standard scenario"}, {"value": "0.0", "module": "A2", "scenario": "Standard scenario"}, {"value": "8.5E-4", "module": "A3", "scenario": "Standard scenario"}, {"value": "8.5E-4", "module": "A1-A3", "scenario": "Standard scenario"}, {"value": "0.0", "module": "C1", "scenario": "Standard scenario"}, {"value": "0.0", "module": "C2", "scenario": "Standard scenario"}, {"value": "0.05", "module": "C3", "scenario": "Standard scenario"}, {"value": "0.0", "module": "C4", "scenario": "Standard scenario"}, {"value": "0.0", "module": "D", "scenario": "Standard scenario"}, {"name": "referenceToUnitGroupDataSet", "value": {"shortDescription": [{"value": "kg", "lang": "en"}], "type": "unit group data set", "refObjectId": "ad38d542-3fe9-439d-9b95-2f5f7752acaf", "version": "30.00.000", "uri": "../unitgroups/ad38d542-3fe9-439d-9b95-2f5f7752acaf.xml"}}]}, "flowProperties": [], "typeOfFlow": "Other flow", "classification": {"classHierarchy": "Größen / Umweltliche Größen / EPD EN 15804 / LCI Indikatoren", "name": "GaBiCategories"}}, {"dataSetInternalID": 9, "referenceToFlowDataSet": {"shortDescription": [{"value": "Non-hazardous waste disposed (NHWD)", "lang": "en"}, {"value": "Entsorgter nicht gefährlicher Abfall (NHWD)", "lang": "de"}, {"value": "Residuos no peligrosos eliminados (NHWD)", "lang": "es"}], "type": "flow data set", "refObjectId": "b29ef66b-e286-4afa-949f-62f1a7b4d7fa", "version": "30.00.000", "uri": "../flows/b29ef66b-e286-4afa-949f-62f1a7b4d7fa.xml"}, "exchange direction": "OUTPUT", "meanAmount": 0.0, "other": {"anies": [{"value": "0.165034235218885", "module": "A1", "scenario": "Standard scenario"}, {"value": "0.0912761966103862", "module": "A2", "scenario": "Standard scenario"}, {"value": "0.0146610851615439", "module": "A3", "scenario": "Standard scenario"}, {"value": "0.2709715169908151", "module": "A1-A3", "scenario": "Standard scenario"}, {"value": "0.0058268363046082", "module": "C1", "scenario": "Standard scenario"}, {"value": "0.0180753915770637", "module": "C2", "scenario": "Standard scenario"}, {"value": "0.0419304", "module": "C3", "scenario": "Standard scenario"}, {"value": "0.1002417", "module": "C4", "scenario": "Standard scenario"}, {"value": "-0.0094484376210428", "module": "D", "scenario": "Standard scenario"}, {"name": "referenceToUnitGroupDataSet", "value": {"shortDescription": [{"value": "kg", "lang": "en"}], "type": "unit group data set", "refObjectId": "ad38d542-3fe9-439d-9b95-2f5f7752acaf", "version": "30.00.000", "uri": "../unitgroups/ad38d542-3fe9-439d-9b95-2f5f7752acaf.xml"}}]}, "flowProperties": [], "typeOfFlow": "Other flow", "classification": {"classHierarchy": "Größen / Umweltliche Größen / EPD EN 15804 / LCI Indikatoren", "name": "GaBiCategories"}}, {"dataSetInternalID": 10, "referenceToFlowDataSet": {"shortDescription": [{"value": "Use of non renewable secondary fuels (NRSF)", "lang": "en"}, {"value": "Nicht erneuerbare Sekundärbrennstoffe (NRSF)", "lang": "de"}, {"value": "Uso de combustibles secundarios no renovables (NRSF)", "lang": "es"}], "type": "flow data set", "refObjectId": "89def144-d39a-4287-b86f-efde453ddcb2", "version": "30.00.000", "uri": "../flows/89def144-d39a-4287-b86f-efde453ddcb2.xml"}, "exchange direction": "INPUT", "meanAmount": 0.0, "other": {"anies": [{"value": "0.0", "module": "A1", "scenario": "Standard scenario"}, {"value": "0.0", "module": "A2", "scenario": "Standard scenario"}, {"value": "0.0", "module": "A3", "scenario": "Standard scenario"}, {"value": "0.0", "module": "A1-A3", "scenario": "Standard scenario"}, {"value": "0.0", "module": "C1", "scenario": "Standard scenario"}, {"value": "0.0", "module": "C2", "scenario": "Standard scenario"}, {"value": "0.0", "module": "C3", "scenario": "Standard scenario"}, {"value": "0.0", "module": "C4", "scenario": "Standard scenario"}, {"value": "0.0", "module": "D", "scenario": "Standard scenario"}, {"name": "referenceToUnitGroupDataSet", "value": {"shortDescription": [{"value": "MJ", "lang": "en"}], "type": "unit group data set", "refObjectId": "93a60a57-a3c8-11da-a746-0800200c9a66", "version": "03.00.000", "uri": "../unitgroups/93a60a57-a3c8-11da-a746-0800200c9a66.xml"}}]}, "flowProperties": [], "typeOfFlow": "Other flow", "classification": {"classHierarchy": "Größen / Umweltliche Größen / EPD EN 15804 / LCI Indikatoren", "name": "GaBiCategories"}}, {"dataSetInternalID": 11, "referenceToFlowDataSet": {"shortDescription": [{"value": "Use of non renewable primary energy (PENRE)", "lang": "en"}, {"value": "Nicht-erneuerbare Primärenergie als Energieträger (PENRE)", "lang": "de"}, {"value": "Uso de energía primaria no renovable, excluyendo los recursos de energía primaria no renovable utilizada como materia prima (PENRE)", "lang": "es"}], "type": "flow data set", "refObjectId": "ac857178-2b45-46ec-892a-a9a4332f0372", "version": "38.00.000", "uri": "../flows/ac857178-2b45-46ec-892a-a9a4332f0372.xml"}, "exchange direction": "INPUT", "meanAmount": 0.0, "other": {"anies": [{"value": "54.6314401048099", "module": "A1", "scenario": "Standard scenario"}, {"value": "1.56498406352345", "module": "A2", "scenario": "Standard scenario"}, {"value": "1.6983340959716", "module": "A3", "scenario": "Standard scenario"}, {"value": "57.89475826430495", "module": "A1-A3", "scenario": "Standard scenario"}, {"value": "5.22637346330632", "module": "C1", "scenario": "Standard scenario"}, {"value": "0.302540708216331", "module": "C2", "scenario": "Standard scenario"}, {"value": "1.8472355", "module": "C3", "scenario": "Standard scenario"}, {"value": "0.0266796", "module": "C4", "scenario": "Standard scenario"}, {"value": "-14.6152654406035", "module": "D", "scenario": "Standard scenario"}, {"name": "referenceToUnitGroupDataSet", "value": {"shortDescription": [{"value": "MJ", "lang": "en"}], "type": "unit group data set", "refObjectId": "93a60a57-a3c8-11da-a746-0800200c9a66", "version": "03.00.000", "uri": "../unitgroups/93a60a57-a3c8-11da-a746-0800200c9a66.xml"}}]}, "flowProperties": [], "typeOfFlow": "Other flow", "classification": {"classHierarchy": "Quantities", "name": "GaBiCategories"}}, {"dataSetInternalID": 12, "referenceToFlowDataSet": {"shortDescription": [{"value": "Use of non renewable primary energy resources used as raw materials (PENRM)", "lang": "en"}, {"value": "Nicht-erneuerbare Primärenergie zur stofflichen Nutzung (PENRM)", "lang": "de"}, {"value": "Uso de la energía primaria no renovable utilizada como materia prima (PENRM)", "lang": "es"}], "type": "flow data set", "refObjectId": "1421caa0-679d-4bf4-b282-0eb850ccae27", "version": "38.00.000", "uri": "../flows/1421caa0-679d-4bf4-b282-0eb850ccae27.xml"}, "exchange direction": "INPUT", "meanAmount": 0.0, "other": {"anies": [{"value": "23.3609856321999", "module": "A1", "scenario": "Standard scenario"}, {"value": "0.0", "module": "A2", "scenario": "Standard scenario"}, {"value": "0.442203319159454", "module": "A3", "scenario": "Standard scenario"}, {"value": "23.803188951359353", "module": "A1-A3", "scenario": "Standard scenario"}, {"value": "0.0", "module": "C1", "scenario": "Standard scenario"}, {"value": "0.0", "module": "C2", "scenario": "Standard scenario"}, {"value": "0.0", "module": "C3", "scenario": "Standard scenario"}, {"value": "0.0", "module": "C4", "scenario": "Standard scenario"}, {"value": "-0.509568034585", "module": "D", "scenario": "Standard scenario"}, {"name": "referenceToUnitGroupDataSet", "value": {"shortDescription": [{"value": "MJ", "lang": "en"}], "type": "unit group data set", "refObjectId": "93a60a57-a3c8-11da-a746-0800200c9a66", "version": "03.00.000", "uri": "../unitgroups/93a60a57-a3c8-11da-a746-0800200c9a66.xml"}}]}, "flowProperties": [], "typeOfFlow": "Other flow", "classification": {"classHierarchy": "Quantities", "name": "GaBiCategories"}}, {"dataSetInternalID": 13, "referenceToFlowDataSet": {"shortDescription": [{"value": "Total use of non-renewable primary energy resources (PENRT)", "lang": "en"}, {"value": "Total nicht erneuerbare Primärenergie (PENRT)", "lang": "de"}, {"value": "Uso total de la energía primaria no renovable (energía primaria y recursos de energía primaria renovable utilizada como materia prima) (PENRT)", "lang": "es"}], "type": "flow data set", "refObjectId": "06159210-646b-4c8d-8583-da9b3b95a6c1", "version": "30.00.000", "uri": "../flows/06159210-646b-4c8d-8583-da9b3b95a6c1.xml"}, "exchange direction": "INPUT", "meanAmount": 0.0, "other": {"anies": [{"value": "77.9924257370099", "module": "A1", "scenario": "Standard scenario"}, {"value": "1.56498406352345", "module": "A2", "scenario": "Standard scenario"}, {"value": "2.14053741513106", "module": "A3", "scenario": "Standard scenario"}, {"value": "81.69794721566441", "module": "A1-A3", "scenario": "Standard scenario"}, {"value": "5.22637346330632", "module": "C1", "scenario": "Standard scenario"}, {"value": "0.302540708216331", "module": "C2", "scenario": "Standard scenario"}, {"value": "1.8472355", "module": "C3", "scenario": "Standard scenario"}, {"value": "0.0266796", "module": "C4", "scenario": "Standard scenario"}, {"value": "-15.1248334751885", "module": "D", "scenario": "Standard scenario"}, {"name": "referenceToUnitGroupDataSet", "value": {"shortDescription": [{"value": "MJ", "lang": "en"}], "type": "unit group data set", "refObjectId": "93a60a57-a3c8-11da-a746-0800200c9a66", "version": "03.00.000", "uri": "../unitgroups/93a60a57-a3c8-11da-a746-0800200c9a66.xml"}}]}, "flowProperties": [], "typeOfFlow": "Other flow", "classification": {"classHierarchy": "Größen / Umweltliche Größen / EPD EN 15804 / LCI Indikatoren", "name": "GaBiCategories"}}, {"dataSetInternalID": 14, "referenceToFlowDataSet": {"shortDescription": [{"value": "Use of renewable primary energy (PERE)", "lang": "en"}, {"value": "Erneuerbare Primärenergie als Energieträger (PERE)", "lang": "de"}, {"value": "Uso de energía primaria renovable excluyendo los recursos de energía primaria renovable utilizada como materia prima (PERE)", "lang": "es"}], "type": "flow data set", "refObjectId": "20f32be5-0398-4288-9b6d-accddd195317", "version": "38.00.000", "uri": "../flows/20f32be5-0398-4288-9b6d-accddd195317.xml"}, "exchange direction": "INPUT", "meanAmount": 0.0, "other": {"anies": [{"value": "0.97834788552345", "module": "A1", "scenario": "Standard scenario"}, {"value": "0.0182591347333312", "module": "A2", "scenario": "Standard scenario"}, {"value": "1.02017265763223", "module": "A3", "scenario": "Standard scenario"}, {"value": "2.0167796778890112", "module": "A1-A3", "scenario": "Standard scenario"}, {"value": "0.026619629479827", "module": "C1", "scenario": "Standard scenario"}, {"value": "0.0035673991811927", "module": "C2", "scenario": "Standard scenario"}, {"value": "0.17796265", "module": "C3", "scenario": "Standard scenario"}, {"value": "4.442E-4", "module": "C4", "scenario": "Standard scenario"}, {"value": "-1.05335836556414", "module": "D", "scenario": "Standard scenario"}, {"name": "referenceToUnitGroupDataSet", "value": {"shortDescription": [{"value": "MJ", "lang": "en"}], "type": "unit group data set", "refObjectId": "93a60a57-a3c8-11da-a746-0800200c9a66", "version": "03.00.000", "uri": "../unitgroups/93a60a57-a3c8-11da-a746-0800200c9a66.xml"}}]}, "flowProperties": [], "typeOfFlow": "Other flow", "classification": {"classHierarchy": "Quantities", "name": "GaBiCategories"}}, {"dataSetInternalID": 15, "referenceToFlowDataSet": {"shortDescription": [{"value": "Use of renewable primary energy resources used as raw materials (PERM)", "lang": "en"}, {"value": "Erneuerbare Primärenergie zur stofflichen Nutzung (PERM)", "lang": "de"}, {"value": "Uso de energía primaria renovable utilizada como materia prima (PERM)", "lang": "es"}], "type": "flow data set", "refObjectId": "fb3ec0de-548d-4508-aea5-00b73bf6f702", "version": "38.00.000", "uri": "../flows/fb3ec0de-548d-4508-aea5-00b73bf6f702.xml"}, "exchange direction": "INPUT", "meanAmount": 0.0, "other": {"anies": [{"value": "0.0", "module": "A1", "scenario": "Standard scenario"}, {"value": "0.0", "module": "A2", "scenario": "Standard scenario"}, {"value": "0.39191586", "module": "A3", "scenario": "Standard scenario"}, {"value": "0.39191586", "module": "A1-A3", "scenario": "Standard scenario"}, {"value": "0.0", "module": "C1", "scenario": "Standard scenario"}, {"value": "0.0", "module": "C2", "scenario": "Standard scenario"}, {"value": "0.0", "module": "C3", "scenario": "Standard scenario"}, {"value": "0.0", "module": "C4", "scenario": "Standard scenario"}, {"value": "0.0", "module": "D", "scenario": "Standard scenario"}, {"name": "referenceToUnitGroupDataSet", "value": {"shortDescription": [{"value": "MJ", "lang": "en"}], "type": "unit group data set", "refObjectId": "93a60a57-a3c8-11da-a746-0800200c9a66", "version": "03.00.000", "uri": "../unitgroups/93a60a57-a3c8-11da-a746-0800200c9a66.xml"}}]}, "flowProperties": [], "typeOfFlow": "Other flow", "classification": {"classHierarchy": "Quantities", "name": "GaBiCategories"}}, {"dataSetInternalID": 16, "referenceToFlowDataSet": {"shortDescription": [{"value": "Total use of renewable primary energy resources (PERT)", "lang": "en"}, {"value": "Total erneuerbare Primärenergie (PERT)", "lang": "de"}, {"value": "Uso total de la energía primaria renovable (energía primaria y recursos de energía primaria renovable utilizada como materia prima) (PERT)", "lang": "es"}], "type": "flow data set", "refObjectId": "53f97275-fa8a-4cdd-9024-65936002acd0", "version": "30.00.000", "uri": "../flows/53f97275-fa8a-4cdd-9024-65936002acd0.xml"}, "exchange direction": "INPUT", "meanAmount": 0.0, "other": {"anies": [{"value": "0.97834788552345", "module": "A1", "scenario": "Standard scenario"}, {"value": "0.0182591347333312", "module": "A2", "scenario": "Standard scenario"}, {"value": "1.41208851763223", "module": "A3", "scenario": "Standard scenario"}, {"value": "2.4086955378890114", "module": "A1-A3", "scenario": "Standard scenario"}, {"value": "0.026619629479827", "module": "C1", "scenario": "Standard scenario"}, {"value": "0.0035673991811927", "module": "C2", "scenario": "Standard scenario"}, {"value": "0.17796265", "module": "C3", "scenario": "Standard scenario"}, {"value": "4.442E-4", "module": "C4", "scenario": "Standard scenario"}, {"value": "-1.05335836556414", "module": "D", "scenario": "Standard scenario"}, {"name": "referenceToUnitGroupDataSet", "value": {"shortDescription": [{"value": "MJ", "lang": "en"}], "type": "unit group data set", "refObjectId": "93a60a57-a3c8-11da-a746-0800200c9a66", "version": "03.00.000", "uri": "../unitgroups/93a60a57-a3c8-11da-a746-0800200c9a66.xml"}}]}, "flowProperties": [], "typeOfFlow": "Other flow", "classification": {"classHierarchy": "Größen / Umweltliche Größen / EPD EN 15804 / LCI Indikatoren", "name": "GaBiCategories"}}, {"dataSetInternalID": 17, "referenceToFlowDataSet": {"shortDescription": [{"value": "Use of renewable secondary fuels (RSF)", "lang": "en"}, {"value": "Erneuerbare Sekundärbrennstoffe (RSF)", "lang": "de"}, {"value": "Uso de combustibles secundarios renovables (RSF)", "lang": "es"}], "type": "flow data set", "refObjectId": "64333088-a55f-4aa2-9a31-c10b07816787", "version": "30.00.000", "uri": "../flows/64333088-a55f-4aa2-9a31-c10b07816787.xml"}, "exchange direction": "INPUT", "meanAmount": 0.0, "other": {"anies": [{"value": "0.0", "module": "A1", "scenario": "Standard scenario"}, {"value": "0.0", "module": "A2", "scenario": "Standard scenario"}, {"value": "0.0", "module": "A3", "scenario": "Standard scenario"}, {"value": "0.0", "module": "A1-A3", "scenario": "Standard scenario"}, {"value": "0.0", "module": "C1", "scenario": "Standard scenario"}, {"value": "0.0", "module": "C2", "scenario": "Standard scenario"}, {"value": "0.0", "module": "C3", "scenario": "Standard scenario"}, {"value": "0.0", "module": "C4", "scenario": "Standard scenario"}, {"value": "0.0", "module": "D", "scenario": "Standard scenario"}, {"name": "referenceToUnitGroupDataSet", "value": {"shortDescription": [{"value": "MJ", "lang": "en"}], "type": "unit group data set", "refObjectId": "93a60a57-a3c8-11da-a746-0800200c9a66", "version": "03.00.000", "uri": "../unitgroups/93a60a57-a3c8-11da-a746-0800200c9a66.xml"}}]}, "flowProperties": [], "typeOfFlow": "Other flow", "classification": {"classHierarchy": "Größen / Umweltliche Größen / EPD EN 15804 / LCI Indikatoren", "name": "GaBiCategories"}}, {"dataSetInternalID": 18, "referenceToFlowDataSet": {"shortDescription": [{"value": "Radioactive waste disposed (RWD)", "lang": "en"}, {"value": "Entsorgter radioaktiver Abfall (RWD)", "lang": "de"}, {"value": "Residuos radiactivos eliminados (RWD)", "lang": "es"}], "type": "flow data set", "refObjectId": "3449546e-52ad-4b39-b809-9fb77cea8ff6", "version": "30.00.000", "uri": "../flows/3449546e-52ad-4b39-b809-9fb77cea8ff6.xml"}, "exchange direction": "OUTPUT", "meanAmount": 0.0, "other": {"anies": [{"value": "3.3669284447E-5", "module": "A1", "scenario": "Standard scenario"}, {"value": "9.6926944793E-6", "module": "A2", "scenario": "Standard scenario"}, {"value": "4.3756726716E-6", "module": "A3", "scenario": "Standard scenario"}, {"value": "4.77376515979E-5", "module": "A1-A3", "scenario": "Standard scenario"}, {"value": "3.41722958186E-5", "module": "C1", "scenario": "Standard scenario"}, {"value": "1.8711655287E-6", "module": "C2", "scenario": "Standard scenario"}, {"value": "6.2455E-6", "module": "C3", "scenario": "Standard scenario"}, {"value": "1.49E-7", "module": "C4", "scenario": "Standard scenario"}, {"value": "-7.1113573181E-6", "module": "D", "scenario": "Standard scenario"}, {"name": "referenceToUnitGroupDataSet", "value": {"shortDescription": [{"value": "kg", "lang": "en"}], "type": "unit group data set", "refObjectId": "ad38d542-3fe9-439d-9b95-2f5f7752acaf", "version": "30.00.000", "uri": "../unitgroups/ad38d542-3fe9-439d-9b95-2f5f7752acaf.xml"}}]}, "flowProperties": [], "typeOfFlow": "Other flow", "classification": {"classHierarchy": "Größen / Umweltliche Größen / EPD EN 15804 / LCI Indikatoren", "name": "GaBiCategories"}}, {"dataSetInternalID": 19, "referenceToFlowDataSet": {"shortDescription": [{"value": "Use of secondary material (SM)", "lang": "en"}, {"value": "Einsatz von Sekundärstoffen (SM)", "lang": "de"}, {"value": "Uso de materiales secundarios (SM)", "lang": "es"}], "type": "flow data set", "refObjectId": "c6a1f35f-2d09-4f54-8dfb-97e502e1ce92", "version": "30.00.000", "uri": "../flows/c6a1f35f-2d09-4f54-8dfb-97e502e1ce92.xml"}, "exchange direction": "INPUT", "meanAmount": 0.0, "other": {"anies": [{"value": "0.017472", "module": "A1", "scenario": "Standard scenario"}, {"value": "0.0", "module": "A2", "scenario": "Standard scenario"}, {"value": "2.97024E-4", "module": "A3", "scenario": "Standard scenario"}, {"value": "0.017769024", "module": "A1-A3", "scenario": "Standard scenario"}, {"value": "0.0", "module": "C1", "scenario": "Standard scenario"}, {"value": "0.0", "module": "C2", "scenario": "Standard scenario"}, {"value": "0.0", "module": "C3", "scenario": "Standard scenario"}, {"value": "0.0", "module": "C4", "scenario": "Standard scenario"}, {"value": "0.0", "module": "D", "scenario": "Standard scenario"}, {"name": "referenceToUnitGroupDataSet", "value": {"shortDescription": [{"value": "kg", "lang": "en"}], "type": "unit group data set", "refObjectId": "ad38d542-3fe9-439d-9b95-2f5f7752acaf", "version": "30.00.000", "uri": "../unitgroups/ad38d542-3fe9-439d-9b95-2f5f7752acaf.xml"}}]}, "flowProperties": [], "typeOfFlow": "Other flow", "classification": {"classHierarchy": "Größen / Umweltliche Größen / EPD EN 15804 / LCI Indikatoren", "name": "GaBiCategories"}}]}, "LCIAResults": {"LCIAResult": [{"referenceToLCIAMethodDataSet": {"shortDescription": [{"value": "Abiotic depletion potential - non-fossil resources (ADPE)", "lang": "en"}, {"value": "Potenzial für die Verknappung abiotischer Ressourcen – nicht fossile Ressourcen (ADPE)", "lang": "de"}], "type": "LCIA method data set", "refObjectId": "b2ad6494-c78d-11e6-9d9d-cec0c932ce01", "version": "01.00.011", "uri": "../lciamethods/b2ad6494-c78d-11e6-9d9d-cec0c932ce01.xml"}, "meanAmount": 0.0, "other": {"anies": [{"value": "2.20005825024E-5", "module": "A1", "scenario": "Standard scenario"}, {"value": "2.4386036203E-6", "module": "A2", "scenario": "Standard scenario"}, {"value": "1.3749172704E-6", "module": "A3", "scenario": "Standard scenario"}, {"value": "2.58141033931E-5", "module": "A1-A3", "scenario": "Standard scenario"}, {"value": "5.483881334E-7", "module": "C1", "scenario": "Standard scenario"}, {"value": "4.787048911E-7", "module": "C2", "scenario": "Standard scenario"}, {"value": "2.879E-6", "module": "C3", "scenario": "Standard scenario"}, {"value": "1.13E-8", "module": "C4", "scenario": "Standard scenario"}, {"value": "-1.0792156126E-6", "module": "D", "scenario": "Standard scenario"}, {"name": "referenceToUnitGroupDataSet", "value": {"shortDescription": [{"value": "kg Sb-eq.", "lang": "en"}], "type": "unit group data set", "refObjectId": "54ccd2d9-a32a-4fc2-923d-f2c8c93e89d4", "version": "30.00.000", "uri": "../unitgroups/54ccd2d9-a32a-4fc2-923d-f2c8c93e89d4.xml"}}]}}, {"referenceToLCIAMethodDataSet": {"shortDescription": [{"value": "Abiotic depletion potential - fossil resources (ADPF)", "lang": "en"}, {"value": "Potenzial für die Verknappung abiotischer Ressourcen – fossile Brennstoffe (ADPF)", "lang": "de"}], "type": "LCIA method data set", "refObjectId": "b2ad6110-c78d-11e6-9d9d-cec0c932ce01", "version": "01.00.011", "uri": "../lciamethods/b2ad6110-c78d-11e6-9d9d-cec0c932ce01.xml"}, "meanAmount": 0.0, "other": {"anies": [{"value": "72.701674629332", "module": "A1", "scenario": "Standard scenario"}, {"value": "1.47400147463307", "module": "A2", "scenario": "Standard scenario"}, {"value": "2.01813020441715", "module": "A3", "scenario": "Standard scenario"}, {"value": "76.19380630838222", "module": "A1-A3", "scenario": "Standard scenario"}, {"value": "4.92137823565623", "module": "C1", "scenario": "Standard scenario"}, {"value": "0.284952224064512", "module": "C2", "scenario": "Standard scenario"}, {"value": "1.7381268", "module": "C3", "scenario": "Standard scenario"}, {"value": "0.0251027", "module": "C4", "scenario": "Standard scenario"}, {"value": "-13.6665518354015", "module": "D", "scenario": "Standard scenario"}, {"name": "referenceToUnitGroupDataSet", "value": {"shortDescription": [{"value": "MJ", "lang": "en"}], "type": "unit group data set", "refObjectId": "93a60a57-a3c8-11da-a746-0800200c9a66", "version": "03.00.000", "uri": "../unitgroups/93a60a57-a3c8-11da-a746-0800200c9a66.xml"}}]}}, {"referenceToLCIAMethodDataSet": {"shortDescription": [{"value": "Acidification potential, Accumulated Exceedance (AP)", "lang": "en"}, {"value": "Versauerungspotenzial, kumulierte Überschreitung (AP)", "lang": "de"}], "type": "LCIA method data set", "refObjectId": "b5c611c6-def3-11e6-bf01-fe55135034f3", "version": "01.03.010", "uri": "../lciamethods/b5c611c6-def3-11e6-bf01-fe55135034f3.xml"}, "meanAmount": 0.0, "other": {"anies": [{"value": "0.0096507714100057", "module": "A1", "scenario": "Standard scenario"}, {"value": "6.375874689362E-4", "module": "A2", "scenario": "Standard scenario"}, {"value": "4.742429348566E-4", "module": "A3", "scenario": "Standard scenario"}, {"value": "0.0107626018137985", "module": "A1-A3", "scenario": "Standard scenario"}, {"value": "0.0037399733759679", "module": "C1", "scenario": "Standard scenario"}, {"value": "1.095775680268E-4", "module": "C2", "scenario": "Standard scenario"}, {"value": "0.00101685", "module": "C3", "scenario": "Standard scenario"}, {"value": "9.25E-6", "module": "C4", "scenario": "Standard scenario"}, {"value": "-8.186682963262E-4", "module": "D", "scenario": "Standard scenario"}, {"name": "referenceToUnitGroupDataSet", "value": {"shortDescription": [{"value": "mol H+-eq.", "lang": "en"}], "type": "unit group data set", "refObjectId": "42e089ac-92bf-4bf2-8ca1-5fc40d18f2ed", "version": "00.01.000", "uri": "../unitgroups/42e089ac-92bf-4bf2-8ca1-5fc40d18f2ed.xml"}}]}}, {"referenceToLCIAMethodDataSet": {"shortDescription": [{"value": "Eutrophication potential - freshwater (EP-freshwater)", "lang": "en"}, {"value": "Eutrophierungspotenzial - Süßwasser (EP-freshwater)", "lang": "de"}], "type": "LCIA method data set", "refObjectId": "b53ec18f-7377-4ad3-86eb-cc3f4f276b2b", "version": "01.00.011", "uri": "../lciamethods/b53ec18f-7377-4ad3-86eb-cc3f4f276b2b.xml"}, "meanAmount": 0.0, "other": {"anies": [{"value": "4.86523906769E-5", "module": "A1", "scenario": "Standard scenario"}, {"value": "9.739300713E-7", "module": "A2", "scenario": "Standard scenario"}, {"value": "5.1602873193E-6", "module": "A3", "scenario": "Standard scenario"}, {"value": "5.47866080675E-5", "module": "A1-A3", "scenario": "Standard scenario"}, {"value": "1.3017501311E-6", "module": "C1", "scenario": "Standard scenario"}, {"value": "1.90591171E-7", "module": "C2", "scenario": "Standard scenario"}, {"value": "6.8115E-6", "module": "C3", "scenario": "Standard scenario"}, {"value": "1.9E-8", "module": "C4", "scenario": "Standard scenario"}, {"value": "-1.9243997713E-6", "module": "D", "scenario": "Standard scenario"}, {"name": "referenceToUnitGroupDataSet", "value": {"shortDescription": [{"value": "kg P-eq.", "lang": "en"}], "type": "unit group data set", "refObjectId": "0429039d-a61d-4590-ba67-aa4a20a810a1", "version": "30.00.000", "uri": "../unitgroups/0429039d-a61d-4590-ba67-aa4a20a810a1.xml"}}]}}, {"referenceToLCIAMethodDataSet": {"shortDescription": [{"value": "Eutrophication potential - marine (EP-marine)", "lang": "en"}, {"value": "Eutrophierungspotenzial - Salzwasser (EP-marine)", "lang": "de"}], "type": "LCIA method data set", "refObjectId": "b5c619fa-def3-11e6-bf01-fe55135034f3", "version": "02.00.011", "uri": "../lciamethods/b5c619fa-def3-11e6-bf01-fe55135034f3.xml"}, "meanAmount": 0.0, "other": {"anies": [{"value": "0.0017763658011874", "module": "A1", "scenario": "Standard scenario"}, {"value": "2.145099552349E-4", "module": "A2", "scenario": "Standard scenario"}, {"value": "1.150392016281E-4", "module": "A3", "scenario": "Standard scenario"}, {"value": "0.0021059149580504003", "module": "A1-A3", "scenario": "Standard scenario"}, {"value": "0.0016510349258229", "module": "C1", "scenario": "Standard scenario"}, {"value": "3.86125072005E-5", "module": "C2", "scenario": "Standard scenario"}, {"value": "2.781E-4", "module": "C3", "scenario": "Standard scenario"}, {"value": "5.6E-6", "module": "C4", "scenario": "Standard scenario"}, {"value": "-2.260819989475E-4", "module": "D", "scenario": "Standard scenario"}, {"name": "referenceToUnitGroupDataSet", "value": {"shortDescription": [{"value": "kg N-eq.", "lang": "en"}], "type": "unit group data set", "refObjectId": "d05bb823-ecdf-4686-8c40-bf1d9257859f", "version": "00.00.003", "uri": "../unitgroups/d05bb823-ecdf-4686-8c40-bf1d9257859f.xml"}}]}}, {"referenceToLCIAMethodDataSet": {"shortDescription": [{"value": "Eutrophication potential - terrestrial (EP-terrestrial)", "lang": "en"}, {"value": "Eutrophierungspotenzial - Land (EP-terrestrial)", "lang": "de"}], "type": "LCIA method data set", "refObjectId": "b5c614d2-def3-11e6-bf01-fe55135034f3", "version": "01.02.010", "uri": "../lciamethods/b5c614d2-def3-11e6-bf01-fe55135034f3.xml"}, "meanAmount": 0.0, "other": {"anies": [{"value": "0.019778168821701", "module": "A1", "scenario": "Standard scenario"}, {"value": "0.0023673502336862", "module": "A2", "scenario": "Standard scenario"}, {"value": "0.0013495638010443", "module": "A3", "scenario": "Standard scenario"}, {"value": "0.0234950828564315", "module": "A1-A3", "scenario": "Standard scenario"}, {"value": "0.0181156693826024", "module": "C1", "scenario": "Standard scenario"}, {"value": "4.257074013997E-4", "module": "C2", "scenario": "Standard scenario"}, {"value": "0.0030951", "module": "C3", "scenario": "Standard scenario"}, {"value": "3.4E-5", "module": "C4", "scenario": "Standard scenario"}, {"value": "-0.0026028572730763", "module": "D", "scenario": "Standard scenario"}, {"name": "referenceToUnitGroupDataSet", "value": {"shortDescription": [{"value": "mol N-eq.", "lang": "en"}], "type": "unit group data set", "refObjectId": "71b4d617-0ec9-4d3f-b65e-e438940c2401", "version": "00.00.003", "uri": "../unitgroups/71b4d617-0ec9-4d3f-b65e-e438940c2401.xml"}}]}}, {"referenceToLCIAMethodDataSet": {"shortDescription": [{"value": "Potential Comparative Toxic Unit for ecosystems (ETP-fw)", "lang": "en"}, {"value": "Potenzielle Toxizitätsvergleichseinheit für Ökosysteme (ETP-fw)", "lang": "de"}], "type": "LCIA method data set", "refObjectId": "05316e7a-b254-4bea-9cf0-6bf33eb5c630", "version": "01.00.003", "uri": "../lciamethods/05316e7a-b254-4bea-9cf0-6bf33eb5c630.xml"}, "meanAmount": 0.0, "other": {"anies": [{"value": "25.9711173593879", "module": "A1", "scenario": "Standard scenario"}, {"value": "1.30579082565681", "module": "A2", "scenario": "Standard scenario"}, {"value": "2.31784003920442", "module": "A3", "scenario": "Standard scenario"}, {"value": "29.59474822424913", "module": "A1-A3", "scenario": "Standard scenario"}, {"value": "2.96671181683226", "module": "C1", "scenario": "Standard scenario"}, {"value": "0.254097918032637", "module": "C2", "scenario": "Standard scenario"}, {"value": "28.6201728", "module": "C3", "scenario": "Standard scenario"}, {"value": "0.0266983", "module": "C4", "scenario": "Standard scenario"}, {"value": "-1.7509780721736", "module": "D", "scenario": "Standard scenario"}, {"name": "referenceToUnitGroupDataSet", "value": {"shortDescription": [{"value": "CTUe", "lang": "en"}], "type": "unit group data set", "refObjectId": "aa959ded-f1eb-4efb-9c5c-2d60be36b3e6", "version": "00.00.003", "uri": "../unitgroups/aa959ded-f1eb-4efb-9c5c-2d60be36b3e6.xml"}}]}}, {"referenceToLCIAMethodDataSet": {"shortDescription": [{"value": "Global Warming Potential - biogenic (GWP-biogenic)", "lang": "en"}, {"value": "Globales Erwärmungspotenzial - biogen (GWP-biogenic)", "lang": "de"}], "type": "LCIA method data set", "refObjectId": "a7ea186c-9749-11ed-a8fc-0242ac120002", "version": "01.00.006", "uri": "../lciamethods/a7ea186c-9749-11ed-a8fc-0242ac120002.xml"}, "meanAmount": 0.0, "other": {"anies": [{"value": "0.0045038062951756", "module": "A1", "scenario": "Standard scenario"}, {"value": "4.28831632528E-5", "module": "A2", "scenario": "Standard scenario"}, {"value": "-0.0526225460147109", "module": "A3", "scenario": "Standard scenario"}, {"value": "-0.0480758565562825", "module": "A1-A3", "scenario": "Standard scenario"}, {"value": "9.94511572545E-5", "module": "C1", "scenario": "Standard scenario"}, {"value": "8.7221807574E-6", "module": "C2", "scenario": "Standard scenario"}, {"value": "3.463E-4", "module": "C3", "scenario": "Standard scenario"}, {"value": "1.14E-5", "module": "C4", "scenario": "Standard scenario"}, {"value": "-0.001124494822184", "module": "D", "scenario": "Standard scenario"}, {"name": "referenceToUnitGroupDataSet", "value": {"shortDescription": [{"value": "kg CO2-eq.", "lang": "en"}], "type": "unit group data set", "refObjectId": "1ebf3012-d0db-4de2-aefd-ef30cedb0be1", "version": "30.00.000", "uri": "../unitgroups/1ebf3012-d0db-4de2-aefd-ef30cedb0be1.xml"}}]}}, {"referenceToLCIAMethodDataSet": {"shortDescription": [{"value": "Global Warming Potential - fossil fuels (GWP-fossil)", "lang": "en"}, {"value": "Globales Erwärmungspotenzial - fossil (GWP-fossil)", "lang": "de"}], "type": "LCIA method data set", "refObjectId": "a7ea19c0-9749-11ed-a8fc-0242ac120002", "version": "01.00.009", "uri": "../lciamethods/a7ea19c0-9749-11ed-a8fc-0242ac120002.xml"}, "meanAmount": 0.0, "other": {"anies": [{"value": "2.361528856768", "module": "A1", "scenario": "Standard scenario"}, {"value": "0.0981726533778464", "module": "A2", "scenario": "Standard scenario"}, {"value": "0.132175671816251", "module": "A3", "scenario": "Standard scenario"}, {"value": "2.591877181962097", "module": "A1-A3", "scenario": "Standard scenario"}, {"value": "0.357572770836371", "module": "C1", "scenario": "Standard scenario"}, {"value": "0.0188935422900024", "module": "C2", "scenario": "Standard scenario"}, {"value": "2.2760354", "module": "C3", "scenario": "Standard scenario"}, {"value": "0.014829", "module": "C4", "scenario": "Standard scenario"}, {"value": "-0.79567455210962", "module": "D", "scenario": "Standard scenario"}, {"name": "referenceToUnitGroupDataSet", "value": {"shortDescription": [{"value": "kg CO2-eq.", "lang": "en"}], "type": "unit group data set", "refObjectId": "1ebf3012-d0db-4de2-aefd-ef30cedb0be1", "version": "30.00.000", "uri": "../unitgroups/1ebf3012-d0db-4de2-aefd-ef30cedb0be1.xml"}}]}}, {"referenceToLCIAMethodDataSet": {"shortDescription": [{"value": "Global Warming Potential - land use and land use change (GWP-luluc)", "lang": "en"}, {"value": "Globales Erwärmungspotenzial - luluc (GWP-luluc)", "lang": "de"}], "type": "LCIA method data set", "refObjectId": "a7ea1ae2-9749-11ed-a8fc-0242ac120002", "version": "01.00.006", "uri": "../lciamethods/a7ea1ae2-9749-11ed-a8fc-0242ac120002.xml"}, "meanAmount": 0.0, "other": {"anies": [{"value": "8.330344882575E-4", "module": "A1", "scenario": "Standard scenario"}, {"value": "3.71290772426E-5", "module": "A2", "scenario": "Standard scenario"}, {"value": "1.379506676319E-4", "module": "A3", "scenario": "Standard scenario"}, {"value": "0.001008114233132", "module": "A1-A3", "scenario": "Standard scenario"}, {"value": "2.81815914583E-5", "module": "C1", "scenario": "Standard scenario"}, {"value": "6.9232308739E-6", "module": "C2", "scenario": "Standard scenario"}, {"value": "1.8305E-4", "module": "C3", "scenario": "Standard scenario"}, {"value": "5.24E-7", "module": "C4", "scenario": "Standard scenario"}, {"value": "-1.163160478561E-4", "module": "D", "scenario": "Standard scenario"}, {"name": "referenceToUnitGroupDataSet", "value": {"shortDescription": [{"value": "kg CO2-eq.", "lang": "en"}], "type": "unit group data set", "refObjectId": "1ebf3012-d0db-4de2-aefd-ef30cedb0be1", "version": "30.00.000", "uri": "../unitgroups/1ebf3012-d0db-4de2-aefd-ef30cedb0be1.xml"}}]}}, {"referenceToLCIAMethodDataSet": {"shortDescription": [{"value": "Global Warming Potential - total (GWP-total)", "lang": "en"}, {"value": "Globales Erwärmungspotenzial - total (GWP-total)", "lang": "de"}], "type": "LCIA method data set", "refObjectId": "a7ea142a-9749-11ed-a8fc-0242ac120002", "version": "04.00.017", "uri": "../lciamethods/a7ea142a-9749-11ed-a8fc-0242ac120002.xml"}, "meanAmount": 0.0, "other": {"anies": [{"value": "2.3668666732929", "module": "A1", "scenario": "Standard scenario"}, {"value": "0.0982526656183418", "module": "A2", "scenario": "Standard scenario"}, {"value": "0.0796910256599798", "module": "A3", "scenario": "Standard scenario"}, {"value": "2.5448103645712217", "module": "A1-A3", "scenario": "Standard scenario"}, {"value": "0.357700403585084", "module": "C1", "scenario": "Standard scenario"}, {"value": "0.0189091877016336", "module": "C2", "scenario": "Standard scenario"}, {"value": "2.27656459999999", "module": "C3", "scenario": "Standard scenario"}, {"value": "0.014841", "module": "C4", "scenario": "Standard scenario"}, {"value": "-0.796915363655735", "module": "D", "scenario": "Standard scenario"}, {"name": "referenceToUnitGroupDataSet", "value": {"shortDescription": [{"value": "kg CO2-eq.", "lang": "en"}], "type": "unit group data set", "refObjectId": "1ebf3012-d0db-4de2-aefd-ef30cedb0be1", "version": "30.00.000", "uri": "../unitgroups/1ebf3012-d0db-4de2-aefd-ef30cedb0be1.xml"}}]}}, {"referenceToLCIAMethodDataSet": {"shortDescription": [{"value": "Potential Comparative Toxic Unit for humans - cancer effects (HTP-c)", "lang": "en"}, {"value": "Potenzielle Toxizitätsvergleichseinheit für den Menschen - kanzerogene Wirkung (HTP-c)", "lang": "de"}], "type": "LCIA method data set", "refObjectId": "2299222a-bbd8-474f-9d4f-4dd1f18aea7c", "version": "01.00.004", "uri": "../lciamethods/2299222a-bbd8-474f-9d4f-4dd1f18aea7c.xml"}, "meanAmount": 0.0, "other": {"anies": [{"value": "6.628518E-10", "module": "A1", "scenario": "Standard scenario"}, {"value": "4.33043E-11", "module": "A2", "scenario": "Standard scenario"}, {"value": "4.6566E-11", "module": "A3", "scenario": "Standard scenario"}, {"value": "7.527221E-10", "module": "A1-A3", "scenario": "Standard scenario"}, {"value": "1.036726E-10", "module": "C1", "scenario": "Standard scenario"}, {"value": "8.2415E-12", "module": "C2", "scenario": "Standard scenario"}, {"value": "4.326E-10", "module": "C3", "scenario": "Standard scenario"}, {"value": "7.0E-13", "module": "C4", "scenario": "Standard scenario"}, {"value": "-7.56276E-11", "module": "D", "scenario": "Standard scenario"}, {"name": "referenceToUnitGroupDataSet", "value": {"shortDescription": [{"value": "CTUh", "lang": "en"}], "type": "unit group data set", "refObjectId": "d4c9523e-2d7e-49fd-8469-998f547d3a70", "version": "00.00.003", "uri": "../unitgroups/d4c9523e-2d7e-49fd-8469-998f547d3a70.xml"}}]}}, {"referenceToLCIAMethodDataSet": {"shortDescription": [{"value": "Potential Comparative Toxic Unit for humans - non-cancer effects (HTP-nc)", "lang": "en"}, {"value": "Potenzielle Toxizitätsvergleichseinheit für den Menschen - nicht kanzerogene Wirkung (HTP-nc)", "lang": "de"}], "type": "LCIA method data set", "refObjectId": "7cfdcfcf-b222-4b26-888a-a55f9fbf7ac8", "version": "01.00.003", "uri": "../lciamethods/7cfdcfcf-b222-4b26-888a-a55f9fbf7ac8.xml"}, "meanAmount": 0.0, "other": {"anies": [{"value": "1.70964261E-8", "module": "A1", "scenario": "Standard scenario"}, {"value": "1.4215405E-9", "module": "A2", "scenario": "Standard scenario"}, {"value": "1.3775579E-9", "module": "A3", "scenario": "Standard scenario"}, {"value": "1.98955245E-8", "module": "A1-A3", "scenario": "Standard scenario"}, {"value": "2.5476637E-9", "module": "C1", "scenario": "Standard scenario"}, {"value": "2.779449E-10", "module": "C2", "scenario": "Standard scenario"}, {"value": "9.0265E-9", "module": "C3", "scenario": "Standard scenario"}, {"value": "1.74E-11", "module": "C4", "scenario": "Standard scenario"}, {"value": "-1.3969015E-9", "module": "D", "scenario": "Standard scenario"}, {"name": "referenceToUnitGroupDataSet", "value": {"shortDescription": [{"value": "CTUh", "lang": "en"}], "type": "unit group data set", "refObjectId": "d4c9523e-2d7e-49fd-8469-998f547d3a70", "version": "00.00.003", "uri": "../unitgroups/d4c9523e-2d7e-49fd-8469-998f547d3a70.xml"}}]}}, {"referenceToLCIAMethodDataSet": {"shortDescription": [{"value": "Potential Human exposure efficiency relative to U235 (IRP)", "lang": "en"}, {"value": "Potenzielle Wirkung durch Exposition des Menschen mit U235 (IRP)", "lang": "de"}], "type": "LCIA method data set", "refObjectId": "b5c632be-def3-11e6-bf01-fe55135034f3", "version": "01.00.012", "uri": "../lciamethods/b5c632be-def3-11e6-bf01-fe55135034f3.xml"}, "meanAmount": 0.0, "other": {"anies": [{"value": "0.03475632226528", "module": "A1", "scenario": "Standard scenario"}, {"value": "0.0061792882979756", "module": "A2", "scenario": "Standard scenario"}, {"value": "0.0035927314975085", "module": "A3", "scenario": "Standard scenario"}, {"value": "0.0445283420607641", "module": "A1-A3", "scenario": "Standard scenario"}, {"value": "0.021089190987853", "module": "C1", "scenario": "Standard scenario"}, {"value": "0.001193908169048", "module": "C2", "scenario": "Standard scenario"}, {"value": "0.0071596", "module": "C3", "scenario": "Standard scenario"}, {"value": "9.82E-5", "module": "C4", "scenario": "Standard scenario"}, {"value": "-0.0050928071937937", "module": "D", "scenario": "Standard scenario"}, {"name": "referenceToUnitGroupDataSet", "value": {"shortDescription": [{"value": "kgBq U235-eq.", "lang": "en"}], "type": "unit group data set", "refObjectId": "456b05bf-1415-44a9-9993-02452f554c09", "version": "00.00.003", "uri": "../unitgroups/456b05bf-1415-44a9-9993-02452f554c09.xml"}}]}}, {"referenceToLCIAMethodDataSet": {"shortDescription": [{"value": "Depletion potential of the stratospheric ozone layer (ODP)", "lang": "en"}, {"value": "Abbaupotenzial der stratosphärischen Ozonschicht (ODP)", "lang": "de"}], "type": "LCIA method data set", "refObjectId": "b5c629d6-def3-11e6-bf01-fe55135034f3", "version": "02.00.013", "uri": "../lciamethods/b5c629d6-def3-11e6-bf01-fe55135034f3.xml"}, "meanAmount": 0.0, "other": {"anies": [{"value": "6.461964E-8", "module": "A1", "scenario": "Standard scenario"}, {"value": "2.1609192E-8", "module": "A2", "scenario": "Standard scenario"}, {"value": "5.5494225E-9", "module": "A3", "scenario": "Standard scenario"}, {"value": "9.17782545E-8", "module": "A1-A3", "scenario": "Standard scenario"}, {"value": "7.72213532E-8", "module": "C1", "scenario": "Standard scenario"}, {"value": "4.1702585E-9", "module": "C2", "scenario": "Standard scenario"}, {"value": "6.9425E-8", "module": "C3", "scenario": "Standard scenario"}, {"value": "3.28E-10", "module": "C4", "scenario": "Standard scenario"}, {"value": "-1.017529273E-7", "module": "D", "scenario": "Standard scenario"}, {"name": "referenceToUnitGroupDataSet", "value": {"shortDescription": [{"value": "kg CFC-11-eq.", "lang": "en"}], "type": "unit group data set", "refObjectId": "d9e957c9-7309-4474-bf3a-7777df6c4e5b", "version": "25.00.000", "uri": "../unitgroups/d9e957c9-7309-4474-bf3a-7777df6c4e5b.xml"}}]}}, {"referenceToLCIAMethodDataSet": {"shortDescription": [{"value": "Potential incidence of disease due to PM emissions (PM)", "lang": "en"}, {"value": "Potenzielles Auftreten von Krankheiten aufgrund von Feinstaubemissionen (PM)", "lang": "de"}], "type": "LCIA method data set", "refObjectId": "b5c602c6-def3-11e6-bf01-fe55135034f3", "version": "02.00.012", "uri": "../lciamethods/b5c602c6-def3-11e6-bf01-fe55135034f3.xml"}, "meanAmount": 0.0, "other": {"anies": [{"value": "8.08741217E-8", "module": "A1", "scenario": "Standard scenario"}, {"value": "8.6604555E-9", "module": "A2", "scenario": "Standard scenario"}, {"value": "6.1334047E-9", "module": "A3", "scenario": "Standard scenario"}, {"value": "9.566798189999999E-8", "module": "A1-A3", "scenario": "Standard scenario"}, {"value": "9.91385722E-8", "module": "C1", "scenario": "Standard scenario"}, {"value": "1.6997309E-9", "module": "C2", "scenario": "Standard scenario"}, {"value": "8.1315E-9", "module": "C3", "scenario": "Standard scenario"}, {"value": "1.74E-10", "module": "C4", "scenario": "Standard scenario"}, {"value": "-3.7697113E-9", "module": "D", "scenario": "Standard scenario"}, {"name": "referenceToUnitGroupDataSet", "value": {"shortDescription": [{"value": "Disease incidence", "lang": "en"}], "type": "unit group data set", "refObjectId": "3883559b-648f-4afc-8ba2-0bd24f3affa3", "version": "00.00.003", "uri": "../unitgroups/3883559b-648f-4afc-8ba2-0bd24f3affa3.xml"}}]}}, {"referenceToLCIAMethodDataSet": {"shortDescription": [{"value": "Photochemical Ozone Creation Potential (POCP)", "lang": "en"}, {"value": "Bildungspotenzial für troposphärisches Ozon (POCP)", "lang": "de"}], "type": "LCIA method data set", "refObjectId": "b5c610fe-def3-11e6-bf01-fe55135034f3", "version": "02.00.015", "uri": "../lciamethods/b5c610fe-def3-11e6-bf01-fe55135034f3.xml"}, "meanAmount": 0.0, "other": {"anies": [{"value": "0.0082603728492939", "module": "A1", "scenario": "Standard scenario"}, {"value": "6.706509145518E-4", "module": "A2", "scenario": "Standard scenario"}, {"value": "4.132336564327E-4", "module": "A3", "scenario": "Standard scenario"}, {"value": "0.0093442574202784", "module": "A1-A3", "scenario": "Standard scenario"}, {"value": "0.0049809123558645", "module": "C1", "scenario": "Standard scenario"}, {"value": "1.215425291224E-4", "module": "C2", "scenario": "Standard scenario"}, {"value": "8.3045E-4", "module": "C3", "scenario": "Standard scenario"}, {"value": "1.3E-5", "module": "C4", "scenario": "Standard scenario"}, {"value": "-8.352436953023E-4", "module": "D", "scenario": "Standard scenario"}, {"name": "referenceToUnitGroupDataSet", "value": {"shortDescription": [{"value": "kg NMVOC-eq.", "lang": "en"}], "type": "unit group data set", "refObjectId": "d27c25f8-fbc1-44c6-b47b-4adbae4199c6", "version": "00.00.003", "uri": "../unitgroups/d27c25f8-fbc1-44c6-b47b-4adbae4199c6.xml"}}]}}, {"referenceToLCIAMethodDataSet": {"shortDescription": [{"value": "Potential Soil quality index (SQP)", "lang": "en"}, {"value": "Potenzieller Bodenqualitätsindex (SQP)", "lang": "de"}], "type": "LCIA method data set", "refObjectId": "b2ad6890-c78d-11e6-9d9d-cec0c932ce01", "version": "01.00.011", "uri": "../lciamethods/b2ad6890-c78d-11e6-9d9d-cec0c932ce01.xml"}, "meanAmount": 0.0, "other": {"anies": [{"value": "3.495622344254", "module": "A1", "scenario": "Standard scenario"}, {"value": "1.25165365374745", "module": "A2", "scenario": "Standard scenario"}, {"value": "6.12148661568903", "module": "A3", "scenario": "Standard scenario"}, {"value": "10.868762613690482", "module": "A1-A3", "scenario": "Standard scenario"}, {"value": "0.628084526914232", "module": "C1", "scenario": "Standard scenario"}, {"value": "0.247122627701304", "module": "C2", "scenario": "Standard scenario"}, {"value": "0.6232392", "module": "C3", "scenario": "Standard scenario"}, {"value": "0.059331", "module": "C4", "scenario": "Standard scenario"}, {"value": "-2.8004539969251", "module": "D", "scenario": "Standard scenario"}, {"name": "referenceToUnitGroupDataSet", "value": {"shortDescription": [{"value": "dimensionless", "lang": "en"}], "type": "unit group data set", "refObjectId": "f130951c-e67f-4f7f-8dd4-665de3974e18", "version": "00.00.004", "uri": "../unitgroups/f130951c-e67f-4f7f-8dd4-665de3974e18.xml"}}]}}, {"referenceToLCIAMethodDataSet": {"shortDescription": [{"value": "Water (user) deprivation potential (WDP)", "lang": "en"}, {"value": "Wasser-Entzugspotenzial (Benutzer) (WDP)", "lang": "de"}], "type": "LCIA method data set", "refObjectId": "b2ad66ce-c78d-11e6-9d9d-cec0c932ce01", "version": "03.00.015", "uri": "../lciamethods/b2ad66ce-c78d-11e6-9d9d-cec0c932ce01.xml"}, "meanAmount": 0.0, "other": {"anies": [{"value": "1.06311019674114", "module": "A1", "scenario": "Standard scenario"}, {"value": "0.0052010269626733", "module": "A2", "scenario": "Standard scenario"}, {"value": "0.0954657091919356", "module": "A3", "scenario": "Standard scenario"}, {"value": "1.1637769328957488", "module": "A1-A3", "scenario": "Standard scenario"}, {"value": "0.0065938788925601", "module": "C1", "scenario": "Standard scenario"}, {"value": "0.0010194720856859", "module": "C2", "scenario": "Standard scenario"}, {"value": "0.11557885", "module": "C3", "scenario": "Standard scenario"}, {"value": "0.001075", "module": "C4", "scenario": "Standard scenario"}, {"value": "-0.0737729461610193", "module": "D", "scenario": "Standard scenario"}, {"name": "referenceToUnitGroupDataSet", "value": {"shortDescription": [{"value": "m3 world eq. deprived", "lang": "en"}], "type": "unit group data set", "refObjectId": "6ae2df01-888e-46c8-b17d-49fa3869b476", "version": "00.00.003", "uri": "../unitgroups/6ae2df01-888e-46c8-b17d-49fa3869b476.xml"}}]}}]}, "otherAttributes": {"{http://www.indata.network/EPD/2019}epd-version": "1.2"}, "version": "1.1"}