{"processInformation": {"dataSetInformation": {"UUID": "98775611-4588-49a7-b539-9beb7492fc4f", "name": {"baseName": [{"value": "ACEMat™", "lang": "en"}]}, "classificationInformation": {"classification": [{"class": [{"value": "Kunststoffe", "level": 0, "classId": "6"}, {"value": "Folien und Vliese", "level": 1, "classId": "6.6"}, {"value": "Technische Textilien", "level": 2, "classId": "6.6.07"}], "name": "OEKOBAU.DAT"}]}, "generalComment": [{"value": "The owner of this EPD shall be liable for the underlying information and evidence. The programme operator Kiwa-Ecobility Experts shall not be liable with respect to manufacturer data, life cycle assessment data and evidence.", "lang": "en"}], "other": {"anies": [{"scenario": [{"description": [{"value": "Almost all the datasets selected for the LCA refer to the RoW as the geographical reference, as there were no specific environmental profiles available. Gold-Joint delivers its product to different countries, so the calculation of transport to construction site (A4) was done by taking the average distance, weighted by the proportion of product shipped to each country. For module A4, a data set for a non-specific truck and a transoceanic ship was used. A scaling method was used to calculate the LCA results for the different ACEMat™ products. The scaling was done on the basis of mass per square meter. As a result of scaling there are results for both the fixed and the scalable part of the scaling function. The fixed part means that this number is the same for each product in the product group and the scalable part is the part that depends on the mass per unit area of the product. In order to calculate the correct number of each environmental impact category for each of the products in the product group, the following calculation should be done: [number fixed part]+([specific mass]*[number scalable part]). The input cardboard tube did not have a linear dependence on the specific mass, so the higher quantity of product available was always taken into account to make the scaling as conservative as possible. The input cardboard tube was not having a linear dependance on the specific mass, thus the higher amount of the product available was always considered for the scaling to be as conservative as possible. For C1 the method and amount of the generic data set 'Polyester weefsel' from chapter 22.46 Grondwapening en grondscheiding of the DuboCalc programme (database version NMD 1.8 - 5.01.14052018) was used. In this generic data set, 0.0013h work per m² of geotextile was assumed."}], "name": "Standard scenario", "default": true}]}]}}, "quantitativeReference": {"referenceToReferenceFlow": [1], "type": "Reference flow(s)"}, "time": {"referenceYear": 2021, "dataSetValidUntil": 2028, "timeRepresentativenessDescription": [{"value": "All process-specific data was collected for the 2021 operating year and is therefore up-to-date. The data is based on the annual average.", "lang": "en"}], "other": {"anies": [{"name": "publicationDateOfEPD", "value": 1703203200000}]}}, "geography": {"locationOfOperationSupplyOrProduction": {"descriptionOfRestrictions": [{"value": "Almost all the datasets selected for the LCA refer to the RoW as the geographical reference, as there were no specific environmental profiles available.", "lang": "en"}], "location": "TW"}}, "technology": {"technologyDescriptionAndIncludedProcesses": [{"value": "ACEMat™ is a Turf Reinforcement Mat (TRM) made of high-strength polypropylene monofilament. With its stable and thick three-dimensional woven structures, ACEMat™ is highly effective in controlling severe erosion problems in steep slopes, barren areas, riverbanks, channels, and areas with heavy rainfall. It interlocks with soil to create a solid base, dissipating run-off and stream erosive forces while protecting the soil surface from water splash and wash. Furthermore, it retains seeds and supports plants when vegetation is required, providing exceptional erosion control and enhanced vegetation performance. The primary material for ACEMat™, PP monofilament, is produced by thoroughly mixing and stirring various plastic pellets, followed by extrusion and stretching processes. After the PP monofilament undergoes the arranging process, it is ready to be fed into the production line for weaving ACEMat™. Weaving is a method of fabric production where two distinct sets of yarn interlace at right angles, forming a longitudinal warp direction (machine direction) and a transversal weft direction (cross-machine direction). Through careful textile design, ACEMat™ displays a rectangular arrangement on its surface. After the fabric undergoes heat shrinking, the yarn forms a three-dimensional rectangular pyramid-like structure. Upon passing visual inspection, the fabric is cut to the required lengths, rolled onto paper tubes for packaging, and then stored in the warehouse. The construction process for the turf reinforcement mat, ACEMat™, can be categorized into the following stages: Preparation of the site; Placement of ACEMat™; Execution of anchorage process; Implementation of hydroseeding process.", "lang": "en"}], "technologicalApplicability": [{"value": "ACEMat™, woven into mesh structures with rectangular pyramid patterns, has shown effectiveness in erosion control and channel protection. This TRM is especially useful in civil engineering for stabilizing slopes. Rain impact can dislodge topsoil, exposing roots and foundations, thus destabilizing slopes. ACEMat™ not only enhances slope filtration and stabilization but also encourages vegetation growth, offering robust soil and rock slope erosion resistance. In environmental restoration, ACEMat™'s ability to promote vegetation and retain soil makes it a key tool, especially given rising concerns over land degradation. Additionally, these mats are used in constructing channels and swales where they reduce erosion and support vegetation. Research is underway to evaluate their potential in optimizing hydraulic efficiency and maintaining channel bed integrity. Their relevance is growing in stormwater management, as they could mitigate runoff and facilitate water infiltration, contributing to sustainable practices, particularly as climate-related challenges like increased precipitation become more common.", "lang": "en"}], "referenceToTechnologyFlowDiagrammOrPicture": [{"shortDescription": [{"value": "Flow chart ACEMat™", "lang": "en"}], "type": "source data set", "refObjectId": "1447ae8a-f9dd-4bee-8967-01651dd40528", "version": "00.00.001"}]}}, "modellingAndValidation": {"LCIMethodAndAllocation": {"typeOfDataSet": "EPD", "other": {"anies": [{"name": "subType", "value": "specific dataset"}]}}, "dataSourcesTreatmentAndRepresentativeness": {"referenceToDataSource": [{"shortDescription": [{"value": "ecoinvent 3.6 database", "lang": "en"}], "type": "source data set", "refObjectId": "766b9973-5ee8-48a2-8098-72c8e20b369f", "version": "00.00.001"}, {"shortDescription": [{"value": "ecoinvent database (general)", "lang": "en"}], "type": "source data set", "refObjectId": "b497a91f-e14b-4b69-8f28-f50eb1576766", "version": "00.03.002"}], "useAdviceForDataSet": [{"value": "The results table shown on the ÖKOBAUDAT refers to the product ACEMat™ R with the specific mass of 0.27 kg/m^2.", "lang": "en"}], "other": {"anies": [{"name": "referenceToOriginalEPD", "value": {"shortDescription": {"value": "ACEMat™ EPD", "defaultValue": "ACEMat™ EPD", "lstrings": [{"lang": "en", "value": "ACEMat™ EPD"}]}, "version": {"version": 1, "majorVersion": 0, "minorVersion": 0, "subMinorVersion": 1, "zero": false, "versionString": "00.00.001"}, "type": "source data set", "uuid": {"uuid": "779d31c2-91ac-48d0-bfb5-0dd4ebca4d04"}, "refObjectId": "779d31c2-91ac-48d0-bfb5-0dd4ebca4d04", "versionAsString": "00.00.001", "resourceURLs": ["https://oekobaudat.de/OEKOBAU.DAT/resource/sources/779d31c2-91ac-48d0-bfb5-0dd4ebca4d04/epd-kiwa-ee-158056-en.pdf?version=00.00.001"]}}]}}, "validation": {"review": [{"reviewDetails": [{"value": "An independent verification in accordance with ISO 14025:2011 has been performed.", "lang": "en"}], "referenceToNameOfReviewerAndInstitution": [{"shortDescription": [{"value": "Elisabet Amat Guasch (External verifier)", "lang": "en"}], "type": "contact data set", "refObjectId": "0b940721-b9a8-4b42-9aae-cba754debb32", "version": "00.00.001"}], "type": "Independent external review"}]}, "complianceDeclarations": {"compliance": [{"referenceToComplianceSystem": {"shortDescription": [{"value": "ISO 14025", "lang": "en"}], "type": "source data set", "refObjectId": "4f2eb655-6e44-4874-a95a-e28f5442cd4d", "version": "00.00.001"}}, {"referenceToComplianceSystem": {"shortDescription": [{"value": "EN 15804+A2", "lang": "de"}, {"value": "EN 15804+A2", "lang": "en"}], "type": "source data set", "refObjectId": "c0016b33-8cf7-415c-ac6e-deba0d21440d", "version": "00.01.000"}}]}}, "administrativeInformation": {"commissionerAndGoal": {"referenceToCommissioner": [{"shortDescription": [{"value": "Gold-Joint Industry Co., Ltd.", "lang": "en"}], "type": "contact data set", "refObjectId": "691fcad9-2d98-41e1-aaf5-7bd40b105840", "version": "00.00.001"}]}, "dataGenerator": {"referenceToPersonOrEntityGeneratingTheDataSet": [{"shortDescription": [{"value": "Kiwa GmbH (Berlin)", "lang": "en"}], "type": "contact data set", "refObjectId": "3ea4a87a-3f88-4633-b7e7-1bbdd272be43", "version": "00.00.001"}]}, "dataEntryBy": {"timeStamp": 1711023206276, "referenceToDataSetFormat": [{"shortDescription": [{"value": "EPD Data Format Extensions v1.2", "lang": "en"}, {"value": "EPD-Datenformaterweiterungen v1.2", "lang": "de"}], "type": "source data set", "refObjectId": "a29449fd-aa2f-4de8-b5d7-4b06b43c6fde", "version": "00.01.000"}, {"shortDescription": [{"value": "ILCD format", "lang": "en"}], "type": "source data set", "refObjectId": "a97a0155-0234-4b87-b4ce-a45da52f2a40", "version": "01.00.000", "uri": "http://lca.jrc.ec.europa.eu/lcainfohub/sample_data/ilcd/sources/ILCD_Format_a97a0155-0234-4b87-b4ce-a45da52f2a40_01.00.000.xml"}], "referenceToPersonOrEntityEnteringTheData": {"shortDescription": [{"value": "Kiwa GmbH (Berlin)", "lang": "en"}], "type": "contact data set", "refObjectId": "3ea4a87a-3f88-4633-b7e7-1bbdd272be43", "version": "00.00.001"}}, "publicationAndOwnership": {"dataSetVersion": "00.00.011", "referenceToRegistrationAuthority": {"shortDescription": [{"value": "Kiwa-Ecobility Experts, Kiwa GmbH (Berlin)", "lang": "en"}], "type": "contact data set", "refObjectId": "eb52a9a8-9d0f-40ce-a5c9-7b78f5615e5a", "version": "00.00.001"}, "registrationNumber": "EPD-Kiwa-EE-158056-EN", "referenceToOwnershipOfDataSet": {"shortDescription": [{"value": "Gold-Joint Industry Co., Ltd.", "lang": "en"}], "type": "contact data set", "refObjectId": "691fcad9-2d98-41e1-aaf5-7bd40b105840", "version": "00.00.001"}, "copyright": true, "licenseType": "Free of charge for all users and uses", "accessRestrictions": [{"value": "None.", "lang": "en"}], "other": {"anies": [{"name": "referenceToPublisher", "value": {"shortDescription": [{"value": "Kiwa-Ecobility Experts, Kiwa GmbH (Berlin)", "lang": "en"}], "type": "contact data set", "refObjectId": "eb52a9a8-9d0f-40ce-a5c9-7b78f5615e5a", "version": "00.00.001"}}]}}}, "exchanges": {"exchange": [{"dataSetInternalID": 1, "referenceToFlowDataSet": {"shortDescription": [{"value": "ACEMat™", "lang": "en"}], "type": "flow data set", "refObjectId": "85d0b3ed-3593-40bf-b6c1-1a6d0b350727", "version": "00.00.002"}, "meanAmount": 1.0, "resultingAmount": 1.0, "referenceFlow": true, "resultingflowAmount": 1.0, "flowProperties": [{"name": [{"lang": "en", "value": "Area"}, {"lang": "de", "value": "Fläche"}], "uuid": "93a60a56-a3c8-19da-a746-0800200c9a66", "referenceFlowProperty": true, "meanValue": 1.0, "referenceUnit": "qm", "unitGroupUUID": "c20a03d7-bd90-4569-bc94-66cfd364dfc8"}], "materialProperties": [{"name": "layer thickness", "value": "0.007", "unit": "m", "unitDescription": "meters"}, {"name": "grammage", "value": "0.27", "unit": "kg/m^2", "unitDescription": "kilograms per square meter"}], "typeOfFlow": "Product flow", "classification": {"classHierarchy": "Kunststoffe / Folien und Vliese / Technische Textilien", "name": "OEKOBAU.DAT"}}, {"dataSetInternalID": 2, "referenceToFlowDataSet": {"shortDescription": [{"value": "Komponenten für die Wiederverwendung (CRU)", "lang": "de"}, {"value": "Components for re-use (CRU)", "lang": "en"}, {"value": "Componentes para su reutilización (CRU)", "lang": "es"}, {"value": "Komponenter för återanvändning (CRU)", "lang": "sv"}], "type": "flow data set", "refObjectId": "a2b32f97-3fc7-4af2-b209-525bc6426f33", "version": "30.00.002"}, "exchange direction": "OUTPUT", "meanAmount": 0.0, "other": {"anies": [{"value": "0.0", "module": "A1", "scenario": "Standard scenario"}, {"value": "0.0", "module": "A2", "scenario": "Standard scenario"}, {"value": "0.0", "module": "A3", "scenario": "Standard scenario"}, {"value": "0.0", "module": "A4", "scenario": "Standard scenario"}, {"value": "0.0", "module": "A5", "scenario": "Standard scenario"}, {"value": "0.0", "module": "C1", "scenario": "Standard scenario"}, {"value": "0.0", "module": "C2", "scenario": "Standard scenario"}, {"value": "0.0", "module": "C3", "scenario": "Standard scenario"}, {"value": "0.0", "module": "C4", "scenario": "Standard scenario"}, {"value": "0.0", "module": "D", "scenario": "Standard scenario"}, {"name": "referenceToUnitGroupDataSet", "value": {"shortDescription": [{"value": "kg"}], "type": "unit group data set", "refObjectId": "ad38d542-3fe9-439d-9b95-2f5f7752acaf", "uri": "../unitgroups/ad38d542-3fe9-439d-9b95-2f5f7752acaf"}}]}, "resolvedFlowVersion": "38.00.000", "flowProperties": [], "typeOfFlow": "Other flow", "classification": {"classHierarchy": "Quantities / Environmental quantities / EPD EN 15804 / LCI indicators", "name": "GaBiCategories"}}, {"dataSetInternalID": 3, "referenceToFlowDataSet": {"shortDescription": [{"value": "Exportierte elektrische Energie (EEE)", "lang": "de"}, {"value": "Exported electrical energy (EEE)", "lang": "en"}, {"value": "Energía exportada electrica (EEE)", "lang": "es"}, {"value": "Exporterad energi – elektrisk (EEE)", "lang": "sv"}], "type": "flow data set", "refObjectId": "4da0c987-2b76-40d6-9e9e-82a017aaaf29", "version": "30.00.002"}, "exchange direction": "OUTPUT", "meanAmount": 0.0, "other": {"anies": [{"value": "0.0", "module": "A1", "scenario": "Standard scenario"}, {"value": "0.0", "module": "A2", "scenario": "Standard scenario"}, {"value": "0.09882862433999975", "module": "A3", "scenario": "Standard scenario"}, {"value": "0.0", "module": "A4", "scenario": "Standard scenario"}, {"value": "0.0", "module": "A5", "scenario": "Standard scenario"}, {"value": "0.0", "module": "C1", "scenario": "Standard scenario"}, {"value": "0.0", "module": "C2", "scenario": "Standard scenario"}, {"value": "0.0", "module": "C3", "scenario": "Standard scenario"}, {"value": "0.0", "module": "C4", "scenario": "Standard scenario"}, {"value": "1.5395754006449973", "module": "D", "scenario": "Standard scenario"}, {"name": "referenceToUnitGroupDataSet", "value": {"shortDescription": [{"value": "MJ"}], "type": "unit group data set", "refObjectId": "93a60a57-a3c8-11da-a746-0800200c9a66", "uri": "../unitgroups/93a60a57-a3c8-11da-a746-0800200c9a66"}}]}, "resolvedFlowVersion": "38.00.000", "flowProperties": [], "typeOfFlow": "Other flow", "classification": {"classHierarchy": "Quantities / Environmental quantities / EPD EN 15804 / LCI indicators", "name": "GaBiCategories"}}, {"dataSetInternalID": 4, "referenceToFlowDataSet": {"shortDescription": [{"value": "Exportierte thermische Energie (EET)", "lang": "de"}, {"value": "Exported thermal energy (EET)", "lang": "en"}, {"value": "Energía exportada termal (EET)", "lang": "es"}, {"value": "Exporterad energi – termisk (EET)", "lang": "sv"}], "type": "flow data set", "refObjectId": "98daf38a-7a79-46d3-9a37-2b7bd0955810", "version": "30.00.002"}, "exchange direction": "OUTPUT", "meanAmount": 0.0, "other": {"anies": [{"value": "0.0", "module": "A1", "scenario": "Standard scenario"}, {"value": "0.0", "module": "A2", "scenario": "Standard scenario"}, {"value": "0.17020485302999971", "module": "A3", "scenario": "Standard scenario"}, {"value": "0.0", "module": "A4", "scenario": "Standard scenario"}, {"value": "0.0", "module": "A5", "scenario": "Standard scenario"}, {"value": "0.0", "module": "C1", "scenario": "Standard scenario"}, {"value": "0.0", "module": "C2", "scenario": "Standard scenario"}, {"value": "0.0", "module": "C3", "scenario": "Standard scenario"}, {"value": "0.0", "module": "C4", "scenario": "Standard scenario"}, {"value": "2.6514909677774994", "module": "D", "scenario": "Standard scenario"}, {"name": "referenceToUnitGroupDataSet", "value": {"shortDescription": [{"value": "MJ"}], "type": "unit group data set", "refObjectId": "93a60a57-a3c8-11da-a746-0800200c9a66", "uri": "../unitgroups/93a60a57-a3c8-11da-a746-0800200c9a66"}}]}, "resolvedFlowVersion": "38.00.000", "flowProperties": [], "typeOfFlow": "Other flow", "classification": {"classHierarchy": "Quantities / Environmental quantities / EPD EN 15804 / LCI indicators", "name": "GaBiCategories"}}, {"dataSetInternalID": 5, "referenceToFlowDataSet": {"shortDescription": [{"value": "Gefährlicher Abfall zur Deponie (HWD)", "lang": "de"}, {"value": "Hazardous waste disposed (HWD)", "lang": "en"}, {"value": "Residuos peligrosos eliminados (HWD)", "lang": "es"}, {"value": "Farligt avfall (HWD)", "lang": "sv"}], "type": "flow data set", "refObjectId": "430f9e0f-59b2-46a0-8e0d-55e0e84948fc", "version": "30.00.002"}, "exchange direction": "OUTPUT", "meanAmount": 0.0, "other": {"anies": [{"value": "2.27988201172E-6", "module": "A1", "scenario": "Standard scenario"}, {"value": "3.4094269620000123E-9", "module": "A2", "scenario": "Standard scenario"}, {"value": "3.0472468828500004E-6", "module": "A3", "scenario": "Standard scenario"}, {"value": "1.4736910782070002E-6", "module": "A4", "scenario": "Standard scenario"}, {"value": "7.3125148748059995E-6", "module": "A5", "scenario": "Standard scenario"}, {"value": "2.5532396357E-6", "module": "C1", "scenario": "Standard scenario"}, {"value": "1.5566114756300002E-7", "module": "C2", "scenario": "Standard scenario"}, {"value": "7.81352183974E-7", "module": "C3", "scenario": "Standard scenario"}, {"value": "2.6375513227000003E-8", "module": "C4", "scenario": "Standard scenario"}, {"value": "-7.680766807205E-6", "module": "D", "scenario": "Standard scenario"}, {"name": "referenceToUnitGroupDataSet", "value": {"shortDescription": [{"value": "kg"}], "type": "unit group data set", "refObjectId": "ad38d542-3fe9-439d-9b95-2f5f7752acaf", "uri": "../unitgroups/ad38d542-3fe9-439d-9b95-2f5f7752acaf"}}]}, "resolvedFlowVersion": "38.00.000", "flowProperties": [], "typeOfFlow": "Other flow", "classification": {"classHierarchy": "Quantities / Environmental quantities / EPD EN 15804 / LCI indicators", "name": "GaBiCategories"}}, {"dataSetInternalID": 6, "referenceToFlowDataSet": {"shortDescription": [{"value": "Stoffe für die Energierückgewinnung (MER)", "lang": "de"}, {"value": "Materials for energy recovery (MER)", "lang": "en"}, {"value": "Materiales para valorización energética (recuperación de energía) (MER)", "lang": "es"}, {"value": "Material till energiåtervinning (MER)", "lang": "sv"}], "type": "flow data set", "refObjectId": "59a9181c-3aaf-46ee-8b13-2b3723b6e447", "version": "30.00.002"}, "exchange direction": "OUTPUT", "meanAmount": 0.0, "other": {"anies": [{"value": "0.0", "module": "A1", "scenario": "Standard scenario"}, {"value": "0.0", "module": "A2", "scenario": "Standard scenario"}, {"value": "0.0", "module": "A3", "scenario": "Standard scenario"}, {"value": "0.0", "module": "A4", "scenario": "Standard scenario"}, {"value": "0.0", "module": "A5", "scenario": "Standard scenario"}, {"value": "0.0", "module": "C1", "scenario": "Standard scenario"}, {"value": "0.0", "module": "C2", "scenario": "Standard scenario"}, {"value": "0.0", "module": "C3", "scenario": "Standard scenario"}, {"value": "0.0", "module": "C4", "scenario": "Standard scenario"}, {"value": "0.0", "module": "D", "scenario": "Standard scenario"}, {"name": "referenceToUnitGroupDataSet", "value": {"shortDescription": [{"value": "kg"}], "type": "unit group data set", "refObjectId": "ad38d542-3fe9-439d-9b95-2f5f7752acaf", "uri": "../unitgroups/ad38d542-3fe9-439d-9b95-2f5f7752acaf"}}]}, "resolvedFlowVersion": "38.00.000", "flowProperties": [], "typeOfFlow": "Other flow", "classification": {"classHierarchy": "Quantities / Environmental quantities / EPD EN 15804 / LCI indicators", "name": "GaBiCategories"}}, {"dataSetInternalID": 7, "referenceToFlowDataSet": {"shortDescription": [{"value": "Stoffe zum Recycling (MFR)", "lang": "de"}, {"value": "Materials for recycling (MFR)", "lang": "en"}, {"value": "Materiales para el reciclaje (MFR)", "lang": "es"}, {"value": "Material till återvinning (MFR)", "lang": "sv"}], "type": "flow data set", "refObjectId": "d7fe48a5-4103-49c8-9aae-b0b5dfdbd6ae", "version": "30.00.002"}, "exchange direction": "OUTPUT", "meanAmount": 0.0, "other": {"anies": [{"value": "0.0", "module": "A1", "scenario": "Standard scenario"}, {"value": "0.0", "module": "A2", "scenario": "Standard scenario"}, {"value": "0.0", "module": "A3", "scenario": "Standard scenario"}, {"value": "0.0", "module": "A4", "scenario": "Standard scenario"}, {"value": "0.01014146", "module": "A5", "scenario": "Standard scenario"}, {"value": "0.0", "module": "C1", "scenario": "Standard scenario"}, {"value": "0.0", "module": "C2", "scenario": "Standard scenario"}, {"value": "0.013829200000000002", "module": "C3", "scenario": "Standard scenario"}, {"value": "0.0", "module": "C4", "scenario": "Standard scenario"}, {"value": "0.0", "module": "D", "scenario": "Standard scenario"}, {"name": "referenceToUnitGroupDataSet", "value": {"shortDescription": [{"value": "kg"}], "type": "unit group data set", "refObjectId": "ad38d542-3fe9-439d-9b95-2f5f7752acaf", "uri": "../unitgroups/ad38d542-3fe9-439d-9b95-2f5f7752acaf"}}]}, "resolvedFlowVersion": "38.00.000", "flowProperties": [], "typeOfFlow": "Other flow", "classification": {"classHierarchy": "Quantities / Environmental quantities / EPD EN 15804 / LCI indicators", "name": "GaBiCategories"}}, {"dataSetInternalID": 8, "referenceToFlowDataSet": {"shortDescription": [{"value": "Einsatz von Süßwasserressourcen (FW)", "lang": "de"}, {"value": "Use of net fresh water (FW)", "lang": "en"}, {"value": "Uso neto de recursos de agua dulce (FW)", "lang": "es"}, {"value": "Användning av sötvatten (FW)", "lang": "sv"}], "type": "flow data set", "refObjectId": "3cf952c8-f3a4-461d-8c96-96456ca62246", "version": "30.00.003"}, "exchange direction": "INPUT", "meanAmount": 0.0, "other": {"anies": [{"value": "0.006019205485878001", "module": "A1", "scenario": "Standard scenario"}, {"value": "1.6388862071800023E-7", "module": "A2", "scenario": "Standard scenario"}, {"value": "0.002558092790254673", "module": "A3", "scenario": "Standard scenario"}, {"value": "1.06808890077341E-4", "module": "A4", "scenario": "Standard scenario"}, {"value": "0.02396284866374197", "module": "A5", "scenario": "Standard scenario"}, {"value": "4.82563994606E-5", "module": "C1", "scenario": "Standard scenario"}, {"value": "7.4825157900680005E-6", "module": "C2", "scenario": "Standard scenario"}, {"value": "7.793052313711771E-4", "module": "C3", "scenario": "Standard scenario"}, {"value": "1.8112759035826006E-5", "module": "C4", "scenario": "Standard scenario"}, {"value": "-6.96585799963895E-4", "module": "D", "scenario": "Standard scenario"}, {"name": "referenceToUnitGroupDataSet", "value": {"shortDescription": [{"value": "m3"}], "type": "unit group data set", "refObjectId": "cd950537-0a98-4044-9ba7-9f9a68d0a504", "uri": "../unitgroups/cd950537-0a98-4044-9ba7-9f9a68d0a504"}}]}, "resolvedFlowVersion": "38.00.000", "flowProperties": [], "typeOfFlow": "Other flow", "classification": {"classHierarchy": "Quantities / Environmental quantities / EPD EN 15804 / LCI indicators", "name": "GaBiCategories"}}, {"dataSetInternalID": 9, "referenceToFlowDataSet": {"shortDescription": [{"value": "Entsorgter nicht gefährlicher Abfall (NHWD)", "lang": "de"}, {"value": "Non hazardous waste dispose (NHWD)", "lang": "en"}, {"value": "Residuos no peligrosos eliminados (NHWD)", "lang": "es"}, {"value": "Icke-farligt avfall (NHWD)", "lang": "sv"}], "type": "flow data set", "refObjectId": "b29ef66b-e286-4afa-949f-62f1a7b4d7fa", "version": "30.00.002"}, "exchange direction": "OUTPUT", "meanAmount": 0.0, "other": {"anies": [{"value": "0.033269694552260004", "module": "A1", "scenario": "Standard scenario"}, {"value": "8.534476887024308E-5", "module": "A2", "scenario": "Standard scenario"}, {"value": "0.0328365486137267", "module": "A3", "scenario": "Standard scenario"}, {"value": "0.032279166099994774", "module": "A4", "scenario": "Standard scenario"}, {"value": "0.09783933514966207", "module": "A5", "scenario": "Standard scenario"}, {"value": "0.0011098735818301", "module": "C1", "scenario": "Standard scenario"}, {"value": "0.003896509580068816", "module": "C2", "scenario": "Standard scenario"}, {"value": "0.010098740851107317", "module": "C3", "scenario": "Standard scenario"}, {"value": "0.06931309942771308", "module": "C4", "scenario": "Standard scenario"}, {"value": "-0.00341926964119569", "module": "D", "scenario": "Standard scenario"}, {"name": "referenceToUnitGroupDataSet", "value": {"shortDescription": [{"value": "kg"}], "type": "unit group data set", "refObjectId": "ad38d542-3fe9-439d-9b95-2f5f7752acaf", "uri": "../unitgroups/ad38d542-3fe9-439d-9b95-2f5f7752acaf"}}]}, "resolvedFlowVersion": "38.00.000", "flowProperties": [], "typeOfFlow": "Other flow", "classification": {"classHierarchy": "Quantities / Environmental quantities / EPD EN 15804 / LCI indicators", "name": "GaBiCategories"}}, {"dataSetInternalID": 10, "referenceToFlowDataSet": {"shortDescription": [{"value": "Nicht-erneuerbare Primärenergie als Energieträger (PENRE)", "lang": "de"}, {"value": "Use of non renewable primary energy (PENRE)", "lang": "en"}, {"value": "Uso de energía primaria no renovable, excluyendo los recursos de energía primaria no renovable utilizada como materia prima (PENRE)", "lang": "es"}, {"value": "Icke förnybar primärenergi - använd som energibärare (PENRE)", "lang": "sv"}], "type": "flow data set", "refObjectId": "ac857178-2b45-46ec-892a-a9a4332f0372", "version": "30.00.002"}, "exchange direction": "INPUT", "meanAmount": 0.0, "other": {"anies": [{"value": "10.712094670509975", "module": "A1", "scenario": "Standard scenario"}, {"value": "0.0014284762079140416", "module": "A2", "scenario": "Standard scenario"}, {"value": "8.115916015200622", "module": "A3", "scenario": "Standard scenario"}, {"value": "0.7883537932698219", "module": "A4", "scenario": "Standard scenario"}, {"value": "17.18180249829934", "module": "A5", "scenario": "Standard scenario"}, {"value": "0.995499707296443", "module": "C1", "scenario": "Standard scenario"}, {"value": "0.0652186572500933", "module": "C2", "scenario": "Standard scenario"}, {"value": "0.43084566651404826", "module": "C3", "scenario": "Standard scenario"}, {"value": "0.018447905650059163", "module": "C4", "scenario": "Standard scenario"}, {"value": "-7.101684002623212", "module": "D", "scenario": "Standard scenario"}, {"name": "referenceToUnitGroupDataSet", "value": {"shortDescription": [{"value": "MJ"}], "type": "unit group data set", "refObjectId": "93a60a57-a3c8-11da-a746-0800200c9a66", "uri": "../unitgroups/93a60a57-a3c8-11da-a746-0800200c9a66"}}]}, "resolvedFlowVersion": "38.00.000", "flowProperties": [], "typeOfFlow": "Other flow", "classification": {"classHierarchy": "Quantities", "name": "GaBiCategories"}}, {"dataSetInternalID": 11, "referenceToFlowDataSet": {"shortDescription": [{"value": "Nicht-erneuerbare Primärenergie zur stofflichen Nutzung (PENRM)", "lang": "de"}, {"value": "Use of non renewable primary energy resources used as raw materials (PENRM)", "lang": "en"}, {"value": "Uso de la energía primaria no renovable utilizada como materia prima (PENRM)", "lang": "es"}, {"value": "Icke förnybar primärenergi - använd som råmaterial (PENRM)", "lang": "sv"}], "type": "flow data set", "refObjectId": "1421caa0-679d-4bf4-b282-0eb850ccae27", "version": "30.00.001"}, "exchange direction": "INPUT", "meanAmount": 0.0, "other": {"anies": [{"value": "11.629492280199983", "module": "A1", "scenario": "Standard scenario"}, {"value": "0.0", "module": "A2", "scenario": "Standard scenario"}, {"value": "1.183880284009996", "module": "A3", "scenario": "Standard scenario"}, {"value": "0.0", "module": "A4", "scenario": "Standard scenario"}, {"value": "0.6406686282104973", "module": "A5", "scenario": "Standard scenario"}, {"value": "0.0", "module": "C1", "scenario": "Standard scenario"}, {"value": "0.0", "module": "C2", "scenario": "Standard scenario"}, {"value": "0.0", "module": "C3", "scenario": "Standard scenario"}, {"value": "0.0", "module": "C4", "scenario": "Standard scenario"}, {"value": "-0.6166924301999974", "module": "D", "scenario": "Standard scenario"}, {"name": "referenceToUnitGroupDataSet", "value": {"shortDescription": [{"value": "MJ"}], "type": "unit group data set", "refObjectId": "93a60a57-a3c8-11da-a746-0800200c9a66", "uri": "../unitgroups/93a60a57-a3c8-11da-a746-0800200c9a66"}}]}, "resolvedFlowVersion": "38.00.000", "flowProperties": [], "typeOfFlow": "Other flow", "classification": {"classHierarchy": "Quantities", "name": "GaBiCategories"}}, {"dataSetInternalID": 12, "referenceToFlowDataSet": {"shortDescription": [{"value": "Nicht erneuerbare Sekundärbrennstoffe (NRSF)", "lang": "de"}, {"value": "Use of non renewable secondary fuels (NRSF)", "lang": "en"}, {"value": "Uso de combustibles secundarios no renovables (NRSF)", "lang": "es"}, {"value": "Användning av ickeförnybara sekundära bränslen (NRSF)", "lang": "sv"}], "type": "flow data set", "refObjectId": "89def144-d39a-4287-b86f-efde453ddcb2", "version": "30.00.001"}, "exchange direction": "INPUT", "meanAmount": 0.0, "other": {"anies": [{"value": "0.0", "module": "A1", "scenario": "Standard scenario"}, {"value": "0.0", "module": "A2", "scenario": "Standard scenario"}, {"value": "0.0", "module": "A3", "scenario": "Standard scenario"}, {"value": "0.0", "module": "A4", "scenario": "Standard scenario"}, {"value": "0.0", "module": "A5", "scenario": "Standard scenario"}, {"value": "0.0", "module": "C1", "scenario": "Standard scenario"}, {"value": "0.0", "module": "C2", "scenario": "Standard scenario"}, {"value": "0.0", "module": "C3", "scenario": "Standard scenario"}, {"value": "0.0", "module": "C4", "scenario": "Standard scenario"}, {"value": "0.0", "module": "D", "scenario": "Standard scenario"}, {"name": "referenceToUnitGroupDataSet", "value": {"shortDescription": [{"value": "MJ"}], "type": "unit group data set", "refObjectId": "93a60a57-a3c8-11da-a746-0800200c9a66", "uri": "../unitgroups/93a60a57-a3c8-11da-a746-0800200c9a66"}}]}, "resolvedFlowVersion": "38.00.000", "flowProperties": [], "typeOfFlow": "Other flow", "classification": {"classHierarchy": "Quantities / Environmental quantities / EPD EN 15804 / LCI indicators", "name": "GaBiCategories"}}, {"dataSetInternalID": 13, "referenceToFlowDataSet": {"shortDescription": [{"value": "Entsorgter radioaktiver Abfall (RWD)", "lang": "de"}, {"value": "Radioactive waste disposed (RWD)", "lang": "en"}, {"value": "Residuos radiactivos eliminados (RWD)", "lang": "es"}, {"value": "Radioaktivt avfall (RWD) ", "lang": "sv"}], "type": "flow data set", "refObjectId": "3449546e-52ad-4b39-b809-9fb77cea8ff6", "version": "30.00.001"}, "exchange direction": "OUTPUT", "meanAmount": 0.0, "other": {"anies": [{"value": "6.189771662776E-6", "module": "A1", "scenario": "Standard scenario"}, {"value": "8.834895180000036E-9", "module": "A2", "scenario": "Standard scenario"}, {"value": "1.9242855391553003E-5", "module": "A3", "scenario": "Standard scenario"}, {"value": "4.866514149672E-6", "module": "A4", "scenario": "Standard scenario"}, {"value": "1.3008362999598001E-5", "module": "A5", "scenario": "Standard scenario"}, {"value": "6.5090087273E-6", "module": "C1", "scenario": "Standard scenario"}, {"value": "4.0336688567400007E-7", "module": "C2", "scenario": "Standard scenario"}, {"value": "1.4571578017260001E-6", "module": "C3", "scenario": "Standard scenario"}, {"value": "1.0314420104200001E-7", "module": "C4", "scenario": "Standard scenario"}, {"value": "-3.481362447682E-6", "module": "D", "scenario": "Standard scenario"}, {"name": "referenceToUnitGroupDataSet", "value": {"shortDescription": [{"value": "kg"}], "type": "unit group data set", "refObjectId": "ad38d542-3fe9-439d-9b95-2f5f7752acaf", "uri": "../unitgroups/ad38d542-3fe9-439d-9b95-2f5f7752acaf"}}]}, "resolvedFlowVersion": "38.00.000", "flowProperties": [], "typeOfFlow": "Other flow", "classification": {"classHierarchy": "Quantities / Environmental quantities / EPD EN 15804 / LCI indicators", "name": "GaBiCategories"}}, {"dataSetInternalID": 14, "referenceToFlowDataSet": {"shortDescription": [{"value": "Erneuerbare Primärenergie als Energieträger (PERE)", "lang": "de"}, {"value": "Use of renewable primary energy (PERE)", "lang": "en"}, {"value": "Uso de energía primaria renovable excluyendo los recursos de energía primaria renovable utilizada como materia prima (PERE)", "lang": "es"}, {"value": "Förnybar energi - använd som energibärare (PERE)", "lang": "sv"}], "type": "flow data set", "refObjectId": "20f32be5-0398-4288-9b6d-accddd195317", "version": "30.00.001"}, "exchange direction": "INPUT", "meanAmount": 0.0, "other": {"anies": [{"value": "0.2347695214712973", "module": "A1", "scenario": "Standard scenario"}, {"value": "1.6843831973932077E-5", "module": "A2", "scenario": "Standard scenario"}, {"value": "0.39500387025269623", "module": "A3", "scenario": "Standard scenario"}, {"value": "0.0110860983479408", "module": "A4", "scenario": "Standard scenario"}, {"value": "0.4894541504727316", "module": "A5", "scenario": "Standard scenario"}, {"value": "0.0050704056152051", "module": "C1", "scenario": "Standard scenario"}, {"value": "7.690237318612491E-4", "module": "C2", "scenario": "Standard scenario"}, {"value": "0.04098876937051435", "module": "C3", "scenario": "Standard scenario"}, {"value": "3.07134023178685E-4", "module": "C4", "scenario": "Standard scenario"}, {"value": "-0.13833684641809238", "module": "D", "scenario": "Standard scenario"}, {"name": "referenceToUnitGroupDataSet", "value": {"shortDescription": [{"value": "MJ"}], "type": "unit group data set", "refObjectId": "93a60a57-a3c8-11da-a746-0800200c9a66", "uri": "../unitgroups/93a60a57-a3c8-11da-a746-0800200c9a66"}}]}, "resolvedFlowVersion": "38.00.000", "flowProperties": [], "typeOfFlow": "Other flow", "classification": {"classHierarchy": "Quantities", "name": "GaBiCategories"}}, {"dataSetInternalID": 15, "referenceToFlowDataSet": {"shortDescription": [{"value": "Erneuerbare Primärenergie zur stofflichen Nutzung (PERM)", "lang": "de"}, {"value": "Use of renewable primary energy resources used as raw materials (PERM)", "lang": "en"}, {"value": "Uso de energía primaria renovable utilizada como materia prima (PERM)", "lang": "es"}, {"value": "Förnybar energi - använd som råmaterial (PERM)", "lang": "sv"}], "type": "flow data set", "refObjectId": "fb3ec0de-548d-4508-aea5-00b73bf6f702", "version": "30.00.001"}, "exchange direction": "INPUT", "meanAmount": 0.0, "other": {"anies": [{"value": "0.0", "module": "A1", "scenario": "Standard scenario"}, {"value": "0.0", "module": "A2", "scenario": "Standard scenario"}, {"value": "0.0", "module": "A3", "scenario": "Standard scenario"}, {"value": "0.0", "module": "A4", "scenario": "Standard scenario"}, {"value": "0.0", "module": "A5", "scenario": "Standard scenario"}, {"value": "0.0", "module": "C1", "scenario": "Standard scenario"}, {"value": "0.0", "module": "C2", "scenario": "Standard scenario"}, {"value": "0.0", "module": "C3", "scenario": "Standard scenario"}, {"value": "0.0", "module": "C4", "scenario": "Standard scenario"}, {"value": "0.0", "module": "D", "scenario": "Standard scenario"}, {"name": "referenceToUnitGroupDataSet", "value": {"shortDescription": [{"value": "MJ"}], "type": "unit group data set", "refObjectId": "93a60a57-a3c8-11da-a746-0800200c9a66", "uri": "../unitgroups/93a60a57-a3c8-11da-a746-0800200c9a66"}}]}, "resolvedFlowVersion": "38.00.000", "flowProperties": [], "typeOfFlow": "Other flow", "classification": {"classHierarchy": "Quantities", "name": "GaBiCategories"}}, {"dataSetInternalID": 16, "referenceToFlowDataSet": {"shortDescription": [{"value": "Erneuerbare Sekundärbrennstoffe (RSF)", "lang": "de"}, {"value": "Use of renewable secondary fuels (RSF)", "lang": "en"}, {"value": "Uso de combustibles secundarios renovables (RSF)", "lang": "es"}, {"value": "Användning av förnybara sekundära bränslen (RSF)", "lang": "sv"}], "type": "flow data set", "refObjectId": "64333088-a55f-4aa2-9a31-c10b07816787", "version": "30.00.001"}, "exchange direction": "INPUT", "meanAmount": 0.0, "other": {"anies": [{"value": "0.0", "module": "A1", "scenario": "Standard scenario"}, {"value": "0.0", "module": "A2", "scenario": "Standard scenario"}, {"value": "0.0", "module": "A3", "scenario": "Standard scenario"}, {"value": "0.0", "module": "A4", "scenario": "Standard scenario"}, {"value": "0.0", "module": "A5", "scenario": "Standard scenario"}, {"value": "0.0", "module": "C1", "scenario": "Standard scenario"}, {"value": "0.0", "module": "C2", "scenario": "Standard scenario"}, {"value": "0.0", "module": "C3", "scenario": "Standard scenario"}, {"value": "0.0", "module": "C4", "scenario": "Standard scenario"}, {"value": "0.0", "module": "D", "scenario": "Standard scenario"}, {"name": "referenceToUnitGroupDataSet", "value": {"shortDescription": [{"value": "MJ"}], "type": "unit group data set", "refObjectId": "93a60a57-a3c8-11da-a746-0800200c9a66", "uri": "../unitgroups/93a60a57-a3c8-11da-a746-0800200c9a66"}}]}, "resolvedFlowVersion": "38.00.000", "flowProperties": [], "typeOfFlow": "Other flow", "classification": {"classHierarchy": "Quantities / Environmental quantities / EPD EN 15804 / LCI indicators", "name": "GaBiCategories"}}, {"dataSetInternalID": 17, "referenceToFlowDataSet": {"shortDescription": [{"value": "Einsatz von Sekundärstoffen (SM)", "lang": "de"}, {"value": "Use of secondary material (SM)", "lang": "en"}, {"value": "Uso de materiales secundarios (SM)", "lang": "es"}, {"value": "Användning av sekundära material (SM)", "lang": "sv"}], "type": "flow data set", "refObjectId": "c6a1f35f-2d09-4f54-8dfb-97e502e1ce92", "version": "30.00.001"}, "exchange direction": "INPUT", "meanAmount": 0.0, "other": {"anies": [{"value": "0.0", "module": "A1", "scenario": "Standard scenario"}, {"value": "0.0", "module": "A2", "scenario": "Standard scenario"}, {"value": "0.0", "module": "A3", "scenario": "Standard scenario"}, {"value": "0.0", "module": "A4", "scenario": "Standard scenario"}, {"value": "0.0", "module": "A5", "scenario": "Standard scenario"}, {"value": "0.0", "module": "C1", "scenario": "Standard scenario"}, {"value": "0.0", "module": "C2", "scenario": "Standard scenario"}, {"value": "0.0", "module": "C3", "scenario": "Standard scenario"}, {"value": "0.0", "module": "C4", "scenario": "Standard scenario"}, {"value": "0.0", "module": "D", "scenario": "Standard scenario"}, {"name": "referenceToUnitGroupDataSet", "value": {"shortDescription": [{"value": "kg"}], "type": "unit group data set", "refObjectId": "ad38d542-3fe9-439d-9b95-2f5f7752acaf", "uri": "../unitgroups/ad38d542-3fe9-439d-9b95-2f5f7752acaf"}}]}, "resolvedFlowVersion": "38.00.000", "flowProperties": [], "typeOfFlow": "Other flow", "classification": {"classHierarchy": "Quantities / Environmental quantities / EPD EN 15804 / LCI indicators", "name": "GaBiCategories"}}, {"dataSetInternalID": 18, "referenceToFlowDataSet": {"shortDescription": [{"value": "Total nicht erneuerbare Primärenergie (PENRT)", "lang": "de"}, {"value": "Total use of non renewable primary energy resource (PENRT)", "lang": "en"}, {"value": "Uso total de la energía primaria no renovable (energía primaria y recursos de energía primaria renovable utilizada como materia prima) (PENRT)", "lang": "es"}, {"value": "Icke förnybar primärenergi – total (PENRT)", "lang": "sv"}], "type": "flow data set", "refObjectId": "06159210-646b-4c8d-8583-da9b3b95a6c1", "version": "30.00.001"}, "exchange direction": "INPUT", "meanAmount": 0.0, "other": {"anies": [{"value": "22.34158695070974", "module": "A1", "scenario": "Standard scenario"}, {"value": "0.0014284762079140416", "module": "A2", "scenario": "Standard scenario"}, {"value": "9.299796299210616", "module": "A3", "scenario": "Standard scenario"}, {"value": "0.7883537932698219", "module": "A4", "scenario": "Standard scenario"}, {"value": "17.822471126509843", "module": "A5", "scenario": "Standard scenario"}, {"value": "0.995499707296443", "module": "C1", "scenario": "Standard scenario"}, {"value": "0.0652186572500933", "module": "C2", "scenario": "Standard scenario"}, {"value": "0.43084566651404826", "module": "C3", "scenario": "Standard scenario"}, {"value": "0.018447905650059163", "module": "C4", "scenario": "Standard scenario"}, {"value": "-7.718376432823212", "module": "D", "scenario": "Standard scenario"}, {"name": "referenceToUnitGroupDataSet", "value": {"shortDescription": [{"value": "MJ"}], "type": "unit group data set", "refObjectId": "93a60a57-a3c8-11da-a746-0800200c9a66", "uri": "../unitgroups/93a60a57-a3c8-11da-a746-0800200c9a66"}}]}, "resolvedFlowVersion": "38.00.000", "flowProperties": [], "typeOfFlow": "Other flow", "classification": {"classHierarchy": "Quantities / Environmental quantities / EPD EN 15804 / LCI indicators", "name": "GaBiCategories"}}, {"dataSetInternalID": 19, "referenceToFlowDataSet": {"shortDescription": [{"value": "Total erneuerbare Primärenergie (PERT)", "lang": "de"}, {"value": "Total use of renewable primary energy resources (PERT)", "lang": "en"}, {"value": "Uso total de la energía primaria renovable (energía primaria y recursos de energía primaria renovable utilizada como materia prima) (PERT)", "lang": "es"}, {"value": "Förnybar energi – total (PERT)", "lang": "sv"}], "type": "flow data set", "refObjectId": "53f97275-fa8a-4cdd-9024-65936002acd0", "version": "30.00.001"}, "exchange direction": "INPUT", "meanAmount": 0.0, "other": {"anies": [{"value": "0.2347695214712973", "module": "A1", "scenario": "Standard scenario"}, {"value": "1.6843831973932077E-5", "module": "A2", "scenario": "Standard scenario"}, {"value": "0.39500387025269623", "module": "A3", "scenario": "Standard scenario"}, {"value": "0.0110860983479408", "module": "A4", "scenario": "Standard scenario"}, {"value": "0.4894541504727316", "module": "A5", "scenario": "Standard scenario"}, {"value": "0.0050704056152051", "module": "C1", "scenario": "Standard scenario"}, {"value": "7.690237318612491E-4", "module": "C2", "scenario": "Standard scenario"}, {"value": "0.04098876937051435", "module": "C3", "scenario": "Standard scenario"}, {"value": "3.07134023178685E-4", "module": "C4", "scenario": "Standard scenario"}, {"value": "-0.13833684641809238", "module": "D", "scenario": "Standard scenario"}, {"name": "referenceToUnitGroupDataSet", "value": {"shortDescription": [{"value": "MJ"}], "type": "unit group data set", "refObjectId": "93a60a57-a3c8-11da-a746-0800200c9a66", "uri": "../unitgroups/93a60a57-a3c8-11da-a746-0800200c9a66"}}]}, "resolvedFlowVersion": "38.00.000", "flowProperties": [], "typeOfFlow": "Other flow", "classification": {"classHierarchy": "Quantities / Environmental quantities / EPD EN 15804 / LCI indicators", "name": "GaBiCategories"}}]}, "LCIAResults": {"LCIAResult": [{"referenceToLCIAMethodDataSet": {"shortDescription": [{"value": "Potenzial für die Verknappung abiotischer Ressourcen – nicht fossile Ressourcen (ADPE)", "lang": "de"}, {"value": "Abiotic depletion potential - non-fossil resources (ADPE)", "lang": "en"}, {"value": "Abiotisk utarmningspotential icke fossila resurser (ADP-mm)", "lang": "sv"}], "type": "LCIA method data set", "refObjectId": "b2ad6494-c78d-11e6-9d9d-cec0c932ce01", "version": "01.00.012"}, "meanAmount": 0.0, "other": {"anies": [{"value": "6.070234643018001E-6", "module": "A1", "scenario": "Standard scenario"}, {"value": "2.2602530510000056E-9", "module": "A2", "scenario": "Standard scenario"}, {"value": "1.36375968976E-6", "module": "A3", "scenario": "Standard scenario"}, {"value": "8.787914131150001E-7", "module": "A4", "scenario": "Standard scenario"}, {"value": "2.65272538389E-6", "module": "A5", "scenario": "Standard scenario"}, {"value": "1.044548826E-7", "module": "C1", "scenario": "Standard scenario"}, {"value": "1.03194345037E-7", "module": "C2", "scenario": "Standard scenario"}, {"value": "6.666707433750001E-7", "module": "C3", "scenario": "Standard scenario"}, {"value": "7.846695908000001E-9", "module": "C4", "scenario": "Standard scenario"}, {"value": "-3.585241498170001E-7", "module": "D", "scenario": "Standard scenario"}, {"name": "referenceToUnitGroupDataSet", "value": {"shortDescription": [{"value": "kg Sb-Äqv."}], "type": "unit group data set", "refObjectId": "54ccd2d9-a32a-4fc2-923d-f2c8c93e89d4", "uri": "../unitgroups/54ccd2d9-a32a-4fc2-923d-f2c8c93e89d4"}}]}}, {"referenceToLCIAMethodDataSet": {"shortDescription": [{"value": "Potenzial für die Verknappung abiotischer Ressourcen – fossile Brennstoffe (ADPF)", "lang": "de"}, {"value": "Abiotic depletion potential - fossil resources (ADPF)", "lang": "en"}, {"value": "Abiotisk utarmningspotential av fossila resurser (ADP-F)", "lang": "sv"}], "type": "LCIA method data set", "refObjectId": "b2ad6110-c78d-11e6-9d9d-cec0c932ce01", "version": "01.00.012"}, "meanAmount": 0.0, "other": {"anies": [{"value": "20.8266968832", "module": "A1", "scenario": "Standard scenario"}, {"value": "0.0013454304211428132", "module": "A2", "scenario": "Standard scenario"}, {"value": "8.745727678640465", "module": "A3", "scenario": "Standard scenario"}, {"value": "0.742570063877143", "module": "A4", "scenario": "Standard scenario"}, {"value": "16.595118523237748", "module": "A5", "scenario": "Standard scenario"}, {"value": "0.937405378220235", "module": "C1", "scenario": "Standard scenario"}, {"value": "0.06142711023412625", "module": "C2", "scenario": "Standard scenario"}, {"value": "0.40536392883556094", "module": "C3", "scenario": "Standard scenario"}, {"value": "0.017357537656762533", "module": "C4", "scenario": "Standard scenario"}, {"value": "-6.991687846394474", "module": "D", "scenario": "Standard scenario"}, {"name": "referenceToUnitGroupDataSet", "value": {"shortDescription": [{"value": "MJ"}], "type": "unit group data set", "refObjectId": "93a60a57-a3c8-11da-a746-0800200c9a66", "uri": "../unitgroups/93a60a57-a3c8-11da-a746-0800200c9a66"}}]}}, {"referenceToLCIAMethodDataSet": {"shortDescription": [{"value": "Versauerungspotenzial, kumulierte Überschreitung (AP)", "lang": "de"}, {"value": "Acidification potential, Accumulated Exceedance (AP)", "lang": "en"}, {"value": "Försurningspotential på land och vatten (AP)", "lang": "sv"}], "type": "LCIA method data set", "refObjectId": "b5c611c6-def3-11e6-bf01-fe55135034f3", "version": "01.03.011", "uri": "http://lca.jrc.ec.europa.eu/lcainfohub/datasets/elcd/lciamethods/f6cbd466-253f-4145-a4bb-8dae7d266e89.xml"}, "meanAmount": 0.0, "other": {"anies": [{"value": "0.0026530396577010003", "module": "A1", "scenario": "Standard scenario"}, {"value": "5.173814452000013E-7", "module": "A2", "scenario": "Standard scenario"}, {"value": "0.0024408733019426173", "module": "A3", "scenario": "Standard scenario"}, {"value": "5.895545175805051E-4", "module": "A4", "scenario": "Standard scenario"}, {"value": "0.004887473627901245", "module": "A5", "scenario": "Standard scenario"}, {"value": "7.123758811368E-4", "module": "C1", "scenario": "Standard scenario"}, {"value": "2.3621620685643002E-5", "module": "C2", "scenario": "Standard scenario"}, {"value": "2.34835778043236E-4", "module": "C3", "scenario": "Standard scenario"}, {"value": "6.394127227776E-6", "module": "C4", "scenario": "Standard scenario"}, {"value": "-3.9738977457877997E-4", "module": "D", "scenario": "Standard scenario"}, {"name": "referenceToUnitGroupDataSet", "value": {"shortDescription": [{"value": "mol H+ eqv."}], "type": "unit group data set", "refObjectId": "42e089ac-92bf-4bf2-8ca1-5fc40d18f2ed", "uri": "../unitgroups/42e089ac-92bf-4bf2-8ca1-5fc40d18f2ed"}}]}}, {"referenceToLCIAMethodDataSet": {"shortDescription": [{"value": "Eutrophierungspotenzial - Süßwasser (EP-freshwater)", "lang": "de"}, {"value": "Eutrophication potential - freshwater (EP-freshwater)", "lang": "en"}, {"value": "Övergödningspotential sötvatten (EP-fw)", "lang": "sv"}], "type": "LCIA method data set", "refObjectId": "b53ec18f-7377-4ad3-86eb-cc3f4f276b2b", "version": "01.00.012", "uri": "http://lca.jrc.ec.europa.eu/lcainfohub/datasets/elcd/lciamethods/a4630d5b-df2f-48ae-b3f2-5e5257606d68.xml"}, "meanAmount": 0.0, "other": {"anies": [{"value": "1.4221575595442001E-5", "module": "A1", "scenario": "Standard scenario"}, {"value": "8.998952370000017E-10", "module": "A2", "scenario": "Standard scenario"}, {"value": "1.7748214666454E-5", "module": "A3", "scenario": "Standard scenario"}, {"value": "5.922233303160001E-7", "module": "A4", "scenario": "Standard scenario"}, {"value": "1.3642609076159E-5", "module": "A5", "scenario": "Standard scenario"}, {"value": "2.479524059E-7", "module": "C1", "scenario": "Standard scenario"}, {"value": "4.1085711486E-8", "module": "C2", "scenario": "Standard scenario"}, {"value": "1.5660410131119997E-6", "module": "C3", "scenario": "Standard scenario"}, {"value": "1.3149529143000002E-8", "module": "C4", "scenario": "Standard scenario"}, {"value": "-9.100201354140001E-7", "module": "D", "scenario": "Standard scenario"}, {"name": "referenceToUnitGroupDataSet", "value": {"shortDescription": [{"value": "kg P eqv."}], "type": "unit group data set", "refObjectId": "0429039d-a61d-4590-ba67-aa4a20a810a1", "uri": "../unitgroups/0429039d-a61d-4590-ba67-aa4a20a810a1"}}]}}, {"referenceToLCIAMethodDataSet": {"shortDescription": [{"value": "Eutrophierungspotenzial - Salzwasser (EP-marine)", "lang": "de"}, {"value": "Eutrophication potential - marine (EP-marine)", "lang": "en"}, {"value": "Övergödningspotential marin (EP-m)", "lang": "sv"}], "type": "LCIA method data set", "refObjectId": "b5c619fa-def3-11e6-bf01-fe55135034f3", "version": "02.00.012", "uri": "http://lca.jrc.ec.europa.eu/lcainfohub/datasets/elcd/lciamethods/5296e2be-060b-4e50-b033-d45f85f6ac92.xml"}, "meanAmount": 0.0, "other": {"anies": [{"value": "4.5178898761040004E-4", "module": "A1", "scenario": "Standard scenario"}, {"value": "1.8231281397800005E-7", "module": "A2", "scenario": "Standard scenario"}, {"value": "3.3730170095545804E-4", "module": "A3", "scenario": "Standard scenario"}, {"value": "1.4629051658782298E-4", "module": "A4", "scenario": "Standard scenario"}, {"value": "0.0014678828493843049", "module": "A5", "scenario": "Standard scenario"}, {"value": "3.144828430139E-4", "module": "C1", "scenario": "Standard scenario"}, {"value": "8.323692661109E-6", "module": "C2", "scenario": "Standard scenario"}, {"value": "6.4274293602782E-5", "module": "C3", "scenario": "Standard scenario"}, {"value": "3.875448930709E-6", "module": "C4", "scenario": "Standard scenario"}, {"value": "-1.05963963932414E-4", "module": "D", "scenario": "Standard scenario"}, {"name": "referenceToUnitGroupDataSet", "value": {"shortDescription": [{"value": "kg N eqv."}], "type": "unit group data set", "refObjectId": "d05bb823-ecdf-4686-8c40-bf1d9257859f", "uri": "../unitgroups/d05bb823-ecdf-4686-8c40-bf1d9257859f"}}]}}, {"referenceToLCIAMethodDataSet": {"shortDescription": [{"value": "Eutrophierungspotenzial - Land (EP-terrestrial)", "lang": "de"}, {"value": "Eutrophication potential - terrestrial (EP-terrestrial)", "lang": "en"}, {"value": "Övergödningspotential total (EP-T)", "lang": "sv"}], "type": "LCIA method data set", "refObjectId": "b5c614d2-def3-11e6-bf01-fe55135034f3", "version": "01.02.011", "uri": "http://lca.jrc.ec.europa.eu/lcainfohub/datasets/elcd/lciamethods/40054970-5936-477c-9bec-29fa23b1cb77.xml"}, "meanAmount": 0.0, "other": {"anies": [{"value": "0.0050341484944120005", "module": "A1", "scenario": "Standard scenario"}, {"value": "2.0100200664010108E-6", "module": "A2", "scenario": "Standard scenario"}, {"value": "0.0037545861980963686", "module": "A3", "scenario": "Standard scenario"}, {"value": "0.0016307898409348002", "module": "A4", "scenario": "Standard scenario"}, {"value": "0.008619439450195731", "module": "A5", "scenario": "Standard scenario"}, {"value": "0.0034506036919243", "module": "C1", "scenario": "Standard scenario"}, {"value": "9.176968370436001E-5", "module": "C2", "scenario": "Standard scenario"}, {"value": "7.15902217265365E-4", "module": "C3", "scenario": "Standard scenario"}, {"value": "2.3522038322842E-5", "module": "C4", "scenario": "Standard scenario"}, {"value": "-0.0011654540190951372", "module": "D", "scenario": "Standard scenario"}, {"name": "referenceToUnitGroupDataSet", "value": {"shortDescription": [{"value": "mol N eqv."}], "type": "unit group data set", "refObjectId": "71b4d617-0ec9-4d3f-b65e-e438940c2401", "uri": "../unitgroups/71b4d617-0ec9-4d3f-b65e-e438940c2401"}}]}}, {"referenceToLCIAMethodDataSet": {"shortDescription": [{"value": "Globales Erwärmungspotenzial - total (GWP-total)", "lang": "de"}, {"value": "Global Warming Potential - total (GWP-total)", "lang": "en"}, {"value": "Global uppvärmningspotential – Totalt (GWP-T)", "lang": "sv"}], "type": "LCIA method data set", "refObjectId": "6a37f984-a4b3-458a-a20a-64418c145fa2", "version": "04.00.018"}, "meanAmount": 0.0, "other": {"anies": [{"value": "0.6639152941387974", "module": "A1", "scenario": "Standard scenario"}, {"value": "8.928162065201207E-5", "module": "A2", "scenario": "Standard scenario"}, {"value": "0.5949170770397203", "module": "A3", "scenario": "Standard scenario"}, {"value": "0.05026148735188168", "module": "A4", "scenario": "Standard scenario"}, {"value": "1.465417813914318", "module": "A5", "scenario": "Standard scenario"}, {"value": "0.0681334102066827", "module": "C1", "scenario": "Standard scenario"}, {"value": "0.004076250891528643", "module": "C2", "scenario": "Standard scenario"}, {"value": "0.5265733717323923", "module": "C3", "scenario": "Standard scenario"}, {"value": "0.010261937557387432", "module": "C4", "scenario": "Standard scenario"}, {"value": "-0.38618567409455784", "module": "D", "scenario": "Standard scenario"}, {"name": "referenceToUnitGroupDataSet", "value": {"shortDescription": [{"value": "kg CO2-Äqv."}], "type": "unit group data set", "refObjectId": "1ebf3012-d0db-4de2-aefd-ef30cedb0be1", "uri": "../unitgroups/1ebf3012-d0db-4de2-aefd-ef30cedb0be1"}}]}}, {"referenceToLCIAMethodDataSet": {"shortDescription": [{"value": "Globales Erwärmungspotenzial - fossil (GWP-fossil)", "lang": "de"}, {"value": "Global Warming Potential - fossil fuels (GWP-fossil)", "lang": "en"}, {"value": "Global uppvärmningspotential– fossil (GWP-f)", "lang": "sv"}], "type": "LCIA method data set", "refObjectId": "5f635281-343e-44fb-83df-1971b155e6b6", "version": "01.00.011"}, "meanAmount": 0.0, "other": {"anies": [{"value": "0.662980624342", "module": "A1", "scenario": "Standard scenario"}, {"value": "8.920774927642997E-5", "module": "A2", "scenario": "Standard scenario"}, {"value": "0.5972212389374609", "module": "A3", "scenario": "Standard scenario"}, {"value": "0.050209587370163254", "module": "A4", "scenario": "Standard scenario"}, {"value": "1.4471069230835074", "module": "A5", "scenario": "Standard scenario"}, {"value": "0.0681090992069279", "module": "C1", "scenario": "Standard scenario"}, {"value": "0.004072878212378354", "module": "C2", "scenario": "Standard scenario"}, {"value": "0.5264557064401245", "module": "C3", "scenario": "Standard scenario"}, {"value": "0.010253676104675227", "module": "C4", "scenario": "Standard scenario"}, {"value": "-0.38591683381392117", "module": "D", "scenario": "Standard scenario"}, {"name": "referenceToUnitGroupDataSet", "value": {"shortDescription": [{"value": "kg CO2-Äqv."}], "type": "unit group data set", "refObjectId": "1ebf3012-d0db-4de2-aefd-ef30cedb0be1", "uri": "../unitgroups/1ebf3012-d0db-4de2-aefd-ef30cedb0be1"}}]}}, {"referenceToLCIAMethodDataSet": {"shortDescription": [{"value": "Globales Erwärmungspotenzial - biogen (GWP-biogenic)", "lang": "de"}, {"value": "Global Warming Potential - biogenic (GWP-biogenic)", "lang": "en"}, {"value": "Global uppvärmningspotential – biogen (GWP-b)", "lang": "sv"}], "type": "LCIA method data set", "refObjectId": "2356e1ab-0185-4db5-86e5-16de51c7485c", "version": "01.00.007"}, "meanAmount": 0.0, "other": {"anies": [{"value": "7.340355181438001E-4", "module": "A1", "scenario": "Standard scenario"}, {"value": "4.118264868000014E-8", "module": "A2", "scenario": "Standard scenario"}, {"value": "-0.002419734923848789", "module": "A3", "scenario": "Standard scenario"}, {"value": "3.1106024910492E-5", "module": "A4", "scenario": "Standard scenario"}, {"value": "0.018065913990588205", "module": "A5", "scenario": "Standard scenario"}, {"value": "1.89430775723E-5", "module": "C1", "scenario": "Standard scenario"}, {"value": "1.8802392598630004E-6", "module": "C2", "scenario": "Standard scenario"}, {"value": "7.5447063002067E-5", "module": "C3", "scenario": "Standard scenario"}, {"value": "7.899034661435001E-6", "module": "C4", "scenario": "Standard scenario"}, {"value": "-2.44751417004884E-4", "module": "D", "scenario": "Standard scenario"}, {"name": "referenceToUnitGroupDataSet", "value": {"shortDescription": [{"value": "kg CO2-Äqv."}], "type": "unit group data set", "refObjectId": "1ebf3012-d0db-4de2-aefd-ef30cedb0be1", "uri": "../unitgroups/1ebf3012-d0db-4de2-aefd-ef30cedb0be1"}}]}}, {"referenceToLCIAMethodDataSet": {"shortDescription": [{"value": "Globales Erwärmungspotenzial - luluc (GWP-luluc)", "lang": "de"}, {"value": "Global Warming Potential - land use and land use change (GWP-luluc)", "lang": "en"}, {"value": "Global uppvärmningspotential - markanvändning och förändringar i markanvändning (GWP-luluc)", "lang": "sv"}], "type": "LCIA method data set", "refObjectId": "4331bbdb-978a-490d-8707-eeb047f01a55", "version": "01.00.007"}, "meanAmount": 0.0, "other": {"anies": [{"value": "2.0062670257628E-4", "module": "A1", "scenario": "Standard scenario"}, {"value": "3.268872690199998E-8", "module": "A2", "scenario": "Standard scenario"}, {"value": "1.1557221115819801E-4", "module": "A3", "scenario": "Standard scenario"}, {"value": "2.0793933089943E-5", "module": "A4", "scenario": "Standard scenario"}, {"value": "2.44973961877069E-4", "module": "A5", "scenario": "Standard scenario"}, {"value": "5.3679221825E-6", "module": "C1", "scenario": "Standard scenario"}, {"value": "1.492439890427E-6", "module": "C2", "scenario": "Standard scenario"}, {"value": "4.221822926386701E-5", "module": "C3", "scenario": "Standard scenario"}, {"value": "3.6241805077100005E-7", "module": "C4", "scenario": "Standard scenario"}, {"value": "-2.4088863630906E-5", "module": "D", "scenario": "Standard scenario"}, {"name": "referenceToUnitGroupDataSet", "value": {"shortDescription": [{"value": "kg CO2-Äqv."}], "type": "unit group data set", "refObjectId": "1ebf3012-d0db-4de2-aefd-ef30cedb0be1", "uri": "../unitgroups/1ebf3012-d0db-4de2-aefd-ef30cedb0be1"}}]}}, {"referenceToLCIAMethodDataSet": {"shortDescription": [{"value": "Abbaupotenzial der stratosphärischen Ozonschicht (ODP)", "lang": "de"}, {"value": "Depletion potential of the stratospheric ozone layer (ODP)", "lang": "en"}, {"value": "Utarmningspotential för stratosfäriska ozonskiktet - ozonnedbrytning (ODP)", "lang": "sv"}], "type": "LCIA method data set", "refObjectId": "b5c629d6-def3-11e6-bf01-fe55135034f3", "version": "02.00.014", "uri": "http://lca.jrc.ec.europa.eu/lcainfohub/datasets/elcd/lciamethods/8b723200-3d8f-4eec-9e10-444edb029476.xml"}, "meanAmount": 0.0, "other": {"anies": [{"value": "1.2945069419000001E-8", "module": "A1", "scenario": "Standard scenario"}, {"value": "1.9690274999999996E-11", "module": "A2", "scenario": "Standard scenario"}, {"value": "2.4860842873000002E-8", "module": "A3", "scenario": "Standard scenario"}, {"value": "1.0696273614E-8", "module": "A4", "scenario": "Standard scenario"}, {"value": "2.4514050440999998E-8", "module": "A5", "scenario": "Standard scenario"}, {"value": "1.47088292E-8", "module": "C1", "scenario": "Standard scenario"}, {"value": "8.989820940000001E-10", "module": "C2", "scenario": "Standard scenario"}, {"value": "1.5888320069E-8", "module": "C3", "scenario": "Standard scenario"}, {"value": "2.26723259E-10", "module": "C4", "scenario": "Standard scenario"}, {"value": "-4.7154387049E-8", "module": "D", "scenario": "Standard scenario"}, {"name": "referenceToUnitGroupDataSet", "value": {"shortDescription": [{"value": "kg CFC 11-Äquiv."}], "type": "unit group data set", "refObjectId": "d9e957c9-7309-4474-bf3a-7777df6c4e5b", "uri": "../unitgroups/d9e957c9-7309-4474-bf3a-7777df6c4e5b"}}]}}, {"referenceToLCIAMethodDataSet": {"shortDescription": [{"value": "Bildungspotenzial für troposphärisches Ozon (POCP)", "lang": "de"}, {"value": "Photochemical Ozone Creation Potential (POCP)", "lang": "en"}, {"value": "Potential till fotokemisk oxidantbildning – marknära ozon (POCP)", "lang": "sv"}], "type": "LCIA method data set", "refObjectId": "b5c610fe-def3-11e6-bf01-fe55135034f3", "version": "02.00.017", "uri": "http://lca.jrc.ec.europa.eu/lcainfohub/datasets/elcd/lciamethods/ec7836be-83eb-41da-bcda-1a6a3fe2d149.xml"}, "meanAmount": 0.0, "other": {"anies": [{"value": "0.0020853692058932", "module": "A1", "scenario": "Standard scenario"}, {"value": "5.738752055020003E-7", "module": "A2", "scenario": "Standard scenario"}, {"value": "0.001189806345727598", "module": "A3", "scenario": "Standard scenario"}, {"value": "4.46377757633659E-4", "module": "A4", "scenario": "Standard scenario"}, {"value": "0.0028816472999502888", "module": "A5", "scenario": "Standard scenario"}, {"value": "9.487452106409E-4", "module": "C1", "scenario": "Standard scenario"}, {"value": "2.6200905639733006E-5", "module": "C2", "scenario": "Standard scenario"}, {"value": "1.9234979975032702E-4", "module": "C3", "scenario": "Standard scenario"}, {"value": "9.000355378242E-6", "module": "C4", "scenario": "Standard scenario"}, {"value": "-4.1724388782459604E-4", "module": "D", "scenario": "Standard scenario"}, {"name": "referenceToUnitGroupDataSet", "value": {"shortDescription": [{"value": "kg NMVOC eqv."}], "type": "unit group data set", "refObjectId": "d27c25f8-fbc1-44c6-b47b-4adbae4199c6", "uri": "../unitgroups/d27c25f8-fbc1-44c6-b47b-4adbae4199c6"}}]}}, {"referenceToLCIAMethodDataSet": {"shortDescription": [{"value": "Wasser-Entzugspotenzial (Benutzer) (WDP)", "lang": "de"}, {"value": "Water (user) deprivation potential (WDP)", "lang": "en"}, {"value": "Vattenfotavtryck (WDP)", "lang": "sv"}], "type": "LCIA method data set", "refObjectId": "b2ad66ce-c78d-11e6-9d9d-cec0c932ce01", "version": "03.00.016"}, "meanAmount": 0.0, "other": {"anies": [{"value": "0.24448677382421732", "module": "A1", "scenario": "Standard scenario"}, {"value": "4.813539399809997E-6", "module": "A2", "scenario": "Standard scenario"}, {"value": "0.09141621016687274", "module": "A3", "scenario": "Standard scenario"}, {"value": "0.003257851896011154", "module": "A4", "scenario": "Standard scenario"}, {"value": "1.0025248294495446", "module": "A5", "scenario": "Standard scenario"}, {"value": "0.0012559769319162", "module": "C1", "scenario": "Standard scenario"}, {"value": "2.1976745187247403E-4", "module": "C2", "scenario": "Standard scenario"}, {"value": "0.026468491691922825", "module": "C3", "scenario": "Standard scenario"}, {"value": "7.433442855212471E-4", "module": "C4", "scenario": "Standard scenario"}, {"value": "-0.04930513612691918", "module": "D", "scenario": "Standard scenario"}, {"name": "referenceToUnitGroupDataSet", "value": {"shortDescription": [{"value": "m3 world eqv."}], "type": "unit group data set", "refObjectId": "6ae2df01-888e-46c8-b17d-49fa3869b476", "uri": "../unitgroups/6ae2df01-888e-46c8-b17d-49fa3869b476"}}]}}, {"referenceToLCIAMethodDataSet": {"shortDescription": [{"value": "Potenzielles Auftreten von Krankheiten aufgrund von Feinstaubemissionen (PM)", "lang": "de"}, {"value": "Potential incidence of disease due to PM emissions (PM)", "lang": "en"}, {"value": "Potential till utsläpp av partiklar (PM)", "lang": "sv"}], "type": "LCIA method data set", "refObjectId": "b5c602c6-def3-11e6-bf01-fe55135034f3", "version": "02.00.013", "uri": "http://lca.jrc.ec.europa.eu/lcainfohub/datasets/elcd/lciamethods/72ce3013-f678-4c6a-935b-f4752ff8901b.xml"}, "meanAmount": 0.0, "other": {"anies": [{"value": "2.1674069787E-8", "module": "A1", "scenario": "Standard scenario"}, {"value": "8.025428999999989E-12", "module": "A2", "scenario": "Standard scenario"}, {"value": "7.94419421E-9", "module": "A3", "scenario": "Standard scenario"}, {"value": "3.555146184E-9", "module": "A4", "scenario": "Standard scenario"}, {"value": "5.1540582801E-8", "module": "A5", "scenario": "Standard scenario"}, {"value": "1.88835376E-8", "module": "C1", "scenario": "Standard scenario"}, {"value": "3.664107200000001E-10", "module": "C2", "scenario": "Standard scenario"}, {"value": "1.9025347220000003E-9", "module": "C3", "scenario": "Standard scenario"}, {"value": "1.20649898E-10", "module": "C4", "scenario": "Standard scenario"}, {"value": "-1.7065385380000004E-9", "module": "D", "scenario": "Standard scenario"}, {"name": "referenceToUnitGroupDataSet", "value": {"shortDescription": [{"value": "disease incidence"}], "type": "unit group data set", "refObjectId": "3883559b-648f-4afc-8ba2-0bd24f3affa3", "uri": "../unitgroups/3883559b-648f-4afc-8ba2-0bd24f3affa3"}}]}}, {"referenceToLCIAMethodDataSet": {"shortDescription": [{"value": "Potenzielle Wirkung durch Exposition des Menschen mit U235 (IRP)", "lang": "de"}, {"value": "Potential Human exposure efficiency relative to U235 (IRP)", "lang": "en"}, {"value": "Exponeringseffektivitet relaterad till U235 (IR)", "lang": "sv"}], "type": "LCIA method data set", "refObjectId": "b5c632be-def3-11e6-bf01-fe55135034f3", "version": "01.00.013", "uri": "http://lca.jrc.ec.europa.eu/lcainfohub/datasets/elcd/lciamethods/a6f4cbc8-5388-44d6-9a67-53d05684f93e.xml"}, "meanAmount": 0.0, "other": {"anies": [{"value": "0.006680141431458", "module": "A1", "scenario": "Standard scenario"}, {"value": "5.637156811018015E-6", "module": "A2", "scenario": "Standard scenario"}, {"value": "0.021705859972869373", "module": "A3", "scenario": "Standard scenario"}, {"value": "0.003167341445111908", "module": "A4", "scenario": "Standard scenario"}, {"value": "0.013202486683797367", "module": "A5", "scenario": "Standard scenario"}, {"value": "0.0040169887595911", "module": "C1", "scenario": "Standard scenario"}, {"value": "2.5737061344335605E-4", "module": "C2", "scenario": "Standard scenario"}, {"value": "0.001658754807708668", "module": "C3", "scenario": "Standard scenario"}, {"value": "6.792187593809802E-5", "module": "C4", "scenario": "Standard scenario"}, {"value": "-0.002616281823177496", "module": "D", "scenario": "Standard scenario"}, {"name": "referenceToUnitGroupDataSet", "value": {"shortDescription": [{"value": "kBq U235 eqv."}], "type": "unit group data set", "refObjectId": "456b05bf-1415-44a9-9993-02452f554c09", "uri": "../unitgroups/456b05bf-1415-44a9-9993-02452f554c09"}}]}}, {"referenceToLCIAMethodDataSet": {"shortDescription": [{"value": "Potenzielle Toxizitätsvergleichseinheit für Ökosysteme (ETP-fw)", "lang": "de"}, {"value": "Potential Comparative Toxic Unit for ecosystems (ETP-fw)", "lang": "en"}, {"value": "Ecotoxicitet (ETP-fw) ", "lang": "sv"}], "type": "LCIA method data set", "refObjectId": "ee1082d1-b0f7-43ca-a1f0-21e2a4a74511", "version": "01.00.004", "uri": "http://lca.jrc.ec.europa.eu/lcainfohub/datasets/elcd/lciamethods/ee1082d1-b0f7-43ca-a1f0-21e2a4a74511.xml"}, "meanAmount": 0.0, "other": {"anies": [{"value": "7.803966190894", "module": "A1", "scenario": "Standard scenario"}, {"value": "0.0011997487297829047", "module": "A2", "scenario": "Standard scenario"}, {"value": "7.125117798102816", "module": "A3", "scenario": "Standard scenario"}, {"value": "0.6120626426045604", "module": "A4", "scenario": "Standard scenario"}, {"value": "5.66824711505065", "module": "A5", "scenario": "Standard scenario"}, {"value": "0.565087965110908", "module": "C1", "scenario": "Standard scenario"}, {"value": "0.05477585189059291", "module": "C2", "scenario": "Standard scenario"}, {"value": "6.530527859411613", "module": "C3", "scenario": "Standard scenario"}, {"value": "0.01846079119962215", "module": "C4", "scenario": "Standard scenario"}, {"value": "-0.5108479024938746", "module": "D", "scenario": "Standard scenario"}, {"name": "referenceToUnitGroupDataSet", "value": {"shortDescription": [{"value": "CTUe"}], "type": "unit group data set", "refObjectId": "aa959ded-f1eb-4efb-9c5c-2d60be36b3e6", "uri": "../unitgroups/aa959ded-f1eb-4efb-9c5c-2d60be36b3e6"}}]}}, {"referenceToLCIAMethodDataSet": {"shortDescription": [{"value": "Potenzielle Toxizitätsvergleichseinheit für den Menschen - kanzerogene Wirkung (HTP-c)", "lang": "de"}, {"value": "Potential Comparative Toxic Unit for humans - cancer effects (HTP-c)", "lang": "en"}, {"value": "Humantoxicitet – cancer (HTP-c)", "lang": "sv"}], "type": "LCIA method data set", "refObjectId": "2299222a-bbd8-474f-9d4f-4dd1f18aea7c", "version": "01.00.005", "uri": "http://lca.jrc.ec.europa.eu/lcainfohub/datasets/elcd/lciamethods/2299222a-bbd8-474f-9d4f-4dd1f18aea7c.xml"}, "meanAmount": 0.0, "other": {"anies": [{"value": "1.52783198E-10", "module": "A1", "scenario": "Standard scenario"}, {"value": "3.892099999999997E-14", "module": "A2", "scenario": "Standard scenario"}, {"value": "1.5037361100000002E-10", "module": "A3", "scenario": "Standard scenario"}, {"value": "2.0055254000000003E-11", "module": "A4", "scenario": "Standard scenario"}, {"value": "5.80782734E-10", "module": "A5", "scenario": "Standard scenario"}, {"value": "1.97472E-11", "module": "C1", "scenario": "Standard scenario"}, {"value": "1.776667E-12", "module": "C2", "scenario": "Standard scenario"}, {"value": "1.0858437700000001E-10", "module": "C3", "scenario": "Standard scenario"}, {"value": "4.842170000000001E-13", "module": "C4", "scenario": "Standard scenario"}, {"value": "-3.0311208E-11", "module": "D", "scenario": "Standard scenario"}, {"name": "referenceToUnitGroupDataSet", "value": {"shortDescription": [{"value": "CTUh"}], "type": "unit group data set", "refObjectId": "d4c9523e-2d7e-49fd-8469-998f547d3a70", "uri": "../unitgroups/d4c9523e-2d7e-49fd-8469-998f547d3a70"}}]}}, {"referenceToLCIAMethodDataSet": {"shortDescription": [{"value": "Potenzielle Toxizitätsvergleichseinheit für den Menschen - nicht kanzerogene Wirkung (HTP-nc)", "lang": "de"}, {"value": "Potential Comparative Toxic Unit for humans - non-cancer effects (HTP-nc)", "lang": "en"}, {"value": "Humantoxicitet – icke cancer (HTP-nc)", "lang": "sv"}], "type": "LCIA method data set", "refObjectId": "3af763a5-b7a1-48c9-9cee-1f223481fcef", "version": "01.00.004", "uri": "http://lca.jrc.ec.europa.eu/lcainfohub/datasets/elcd/lciamethods/3af763a5-b7a1-48c9-9cee-1f223481fcef.xml"}, "meanAmount": 0.0, "other": {"anies": [{"value": "4.808560627000001E-9", "module": "A1", "scenario": "Standard scenario"}, {"value": "1.312349000000002E-12", "module": "A2", "scenario": "Standard scenario"}, {"value": "4.301874988E-9", "module": "A3", "scenario": "Standard scenario"}, {"value": "6.20373799E-10", "module": "A4", "scenario": "Standard scenario"}, {"value": "4.991016882999999E-9", "module": "A5", "scenario": "Standard scenario"}, {"value": "4.852693E-10", "module": "C1", "scenario": "Standard scenario"}, {"value": "5.9916556E-11", "module": "C2", "scenario": "Standard scenario"}, {"value": "2.09218808E-9", "module": "C3", "scenario": "Standard scenario"}, {"value": "1.2014092000000001E-11", "module": "C4", "scenario": "Standard scenario"}, {"value": "-5.01036358E-10", "module": "D", "scenario": "Standard scenario"}, {"name": "referenceToUnitGroupDataSet", "value": {"shortDescription": [{"value": "CTUh"}], "type": "unit group data set", "refObjectId": "d4c9523e-2d7e-49fd-8469-998f547d3a70", "uri": "../unitgroups/d4c9523e-2d7e-49fd-8469-998f547d3a70"}}]}}, {"referenceToLCIAMethodDataSet": {"shortDescription": [{"value": "Potenzieller Bodenqualitätsindex (SQP)", "lang": "de"}, {"value": "Potential Soil quality index (SQP)", "lang": "en"}, {"value": "Potentiell jordkvalitet index (SQP)", "lang": "sv"}], "type": "LCIA method data set", "refObjectId": "b2ad6890-c78d-11e6-9d9d-cec0c932ce01", "version": "01.00.014"}, "meanAmount": 0.0, "other": {"anies": [{"value": "0.7475223275983973", "module": "A1", "scenario": "Standard scenario"}, {"value": "0.0011668141989545182", "module": "A2", "scenario": "Standard scenario"}, {"value": "1.1515217923965873", "module": "A3", "scenario": "Standard scenario"}, {"value": "0.4726850595796835", "module": "A4", "scenario": "Standard scenario"}, {"value": "1.557335285903842", "module": "A5", "scenario": "Standard scenario"}, {"value": "0.119635147983663", "module": "C1", "scenario": "Standard scenario"}, {"value": "0.05327218955033761", "module": "C2", "scenario": "Standard scenario"}, {"value": "0.14931432246953227", "module": "C3", "scenario": "Standard scenario"}, {"value": "0.041025001298068006", "module": "C4", "scenario": "Standard scenario"}, {"value": "-0.7492351463687161", "module": "D", "scenario": "Standard scenario"}, {"name": "referenceToUnitGroupDataSet", "value": {"shortDescription": [{"value": "dimensionless"}], "type": "unit group data set", "refObjectId": "f130951c-e67f-4f7f-8dd4-665de3974e18", "uri": "../unitgroups/f130951c-e67f-4f7f-8dd4-665de3974e18"}}]}}]}, "otherAttributes": {"{http://www.okworx.com/ILCD/Extensions/2018/Profile}profile": "EN_15804_A2", "{http://www.indata.network/EPD/2019}epd-version": "1.2"}, "version": "1.1"}