{"processInformation": {"dataSetInformation": {"UUID": "a6d60a75-7a4e-4dfc-87cc-fd40f68d279a", "name": {"baseName": [{"value": "Dachziegel (inklusive Zubehör)", "lang": "de"}, {"value": "Roofing tiles (including accessories)", "lang": "en"}], "functionalUnitFlowProperties": [{"lang": "de"}]}, "classificationInformation": {"classification": [{"class": [{"value": "Mineralische Baustoffe", "level": 0, "classId": "1"}, {"value": "Steine und Elemente", "level": 1, "classId": "1.3"}, {"value": "Dachziegel", "level": 2, "classId": "1.3.10"}], "name": "OEKOBAU.DAT"}, {"class": [{"value": "02 Bauprodukte", "level": 0}, {"value": "Bedachungen", "level": 1}, {"value": "Dachziegel", "level": 2}], "name": "IBUCategories"}]}, "generalComment": [{"value": "Es werden Tondachziegel inkl. des keramischen Zubehörs der Mitglieder des Bundesverbandes der \n\nDeutschen Ziegelindustrie e. V. bilanziert. Es handelt sich um Flächenziegel, Formziegel und Zubehör (auch für die Fassade geeignet). \n\nDie verschiedenen Produkte unterscheiden sich lediglich in Form und Farbe (Engobe, Glasur). Die maßgebliche Zusammensetzung, d. h. der Ton­ und Lehmanteil, ist weitgehend einheitlich. \n\n\nFür das Inverkehrbringen des Produkts in der EU/EFTA (mit Ausnahme der Schweiz) gilt die Verordnung (EU) Nr. 305/2011(CPR). Das Produkt benötigt eine Leistungserklärung unter Berücksichtigung der DIN EN 1304:2013­08 ­\n\nDachziegel und Formziegel- Begriffe und\n\n\n\nProduktanforderungen und die CE- Kennzeichnung. Für die Verwendung gelten die jeweiligen nationalen Bestimmungen, in Deutschland die Fachregeln des Deutschen Dachdeckerhandwerks sowie die Herstellerangaben", "lang": "de"}, {"value": "Clay roofing tiles, including ceramic accessories, of the members of the Bundesverband der Deutschen Ziegelindustrie e. V. are modelled. This involves flat tiles, shaped tiles and accessories (also suitable for facades).\n\nThe various products are only distinguished in terms of shape and colour (engobe, glaze). The relevant composition, i.e. clay and loam content, is largely uniform.\n\n (EU) Directive No. 305/2011 (CPR) applies for placing the product on the market in the EU/EFTA (with the exception of Switzerland). The product requires a Declaration of Performance taking consideration of the DIN EN 1304:2013-08 – Clay roofing tiles and fittings – Product definitions and specifications, and CE marking. Use is governed by the respective national provisions; in Germany: the rules of the German roofing trade and information supplied by the manufacturer.", "lang": "en"}], "other": {"anies": [{"scenario": [{"description": [{"value": "1", "lang": "de"}, {"value": "1", "lang": "en"}], "name": "S1"}]}]}}, "quantitativeReference": {"referenceToReferenceFlow": [0]}, "time": {"referenceYear": 2021, "dataSetValidUntil": 2026, "other": {"anies": [{"name": "publicationDateOfEPD", "value": 1636934400000}]}}, "geography": {"locationOfOperationSupplyOrProduction": {"location": "DE"}}, "technology": {"technologyDescriptionAndIncludedProcesses": [{"value": "Grubenbetrieb Die Hauptbestandteile (Lehm und Ton) werden im Tagebaubetrieb abgebaut. Der Abbau erfolgt nach Abziehen des Oberbodens und ggf. Bearbeitung von archäologischen Fundstellen in der Regel mit Löffelbaggern. Der Transport wird je nach Straßenverhältnissen mit geeigneten Lkw durchgeführt. Bei kurzen Entfernungen können Bandstraßen zum Einsatz kommen. Wenn die Gruben erschöpft sind, werden sie entsprechend den Vorlagen des Naturschutzes rekultiviert und ggf. der vorherigen Nutzung wieder zugeführt. Rohstoffaufbereitung Die einzelnen Rohstoffkomponenten werden beprobt und im Labor auf ihre keramischen Eigenschaften und ihre mineralogischen und chemischen Zusammensetzungen hin analysiert. In der Aufbereitung werden die Komponenten entsprechend ihrer keramischen Eigenschaften zur Betriebsmasse vereint, homogenisiert und gelagert. Formgebung Die Betriebsmasse wird in Strangpressen unter Vakuum zu Batzen verpresst, die anschließend in Revolver­ oder Drehtischpressen mittels Gipsformen zur Ziegelform verpresst werden. Biberschwanzziegel werden nur stranggezogen. Verschiedene Parameter wie Pressenvakuum, Batzeneigenschaften (Feuchte, Plastizität und Gewicht) werden regelmäßig kontrolliert. Überschüssige Betriebsmasse und fehlerhafte Pressungen werden vollständig in den Massekreislauf zurückgeführt. Trocknung Das Trocknen dient als Vorbereitung des plastischen Dachziegels für den darauffolgenden Brennvorgang und erfolgt je nach Modell über 1 – 2 Tage bei ca. 60 – 120 °C. Aufgrund des Schwindungsverhaltens reagiert das keramische Material sehr empfindlich und muss deshalb unter definierten Bedingungen getrocknet werden. Verschiedene Trocknungsparameter sowie die Restfeuchte werden ständig kontrolliert. Aussortierte getrocknete Ziegel (Trockenbruch) werden in der Rohstoffaufbereitung wieder der Betriebsmasse zugeführt. Farbgebung Nach Bedarf werden auf die getrockneten Dachziegel Engoben oder Glasuren aufgetragen. Die Dichte der Engoben/Glasuren sowie die Auftragsstärke werden regelmäßig kontrolliert. Anfallende Reste und das Waschwasser werden aufbereitet und dem Rohstoffkreislauf zugeführt. Brennen Die Ziegel werden in Tunnel­ und Herdwagenöfen unter Verwendung von Erdgas bei ca. 1000 – 1200 °C gebrannt. Die Brenndauer inkl. Aufheiz­ und Abkühlphase beträgt ca. 1 –2 Tage. Durch den Brand erhalten die Ziegel ihre keramischen Eigenschaften, die sie langlebig und beständig machen. Hydrophobierung Zur Verringerung der Wasseraufnahmefähigkeit werden manche Ziegel vor dem Verpacken in einem Tauchbad oberflächlich hydrophobiert. Qualitätskontrolle Die geforderten keramischen Qualitätseigenschaften nach EN 1304 und die einzuhaltenden Produktmaße werden in der werkseigenen Produktionskontrolle (WPK) regelmäßig intern kontrolliert und zusätzlich mindestens jährlich extern überwacht. \nDeklarierte Einheit: \nDie Deklaration bezieht sich auf die Herstellung von 1 m² Dachziegel (40 kg/m²)", "lang": "de"}, {"value": "Pit operation The main components (loam and clay) are extracted in opencast mines. After the topsoil has been removed and, if necessary, archaeological sites have been processed, extraction is usually carried out with excavators. Depending on the road conditions, transport entails the use of suitable trucks. Conveyor belts can be used for short distances. When the pits are exhausted, they are recultivated in accordance with nature conservation guidelines and, if necessary, returned to their previous use. Processing raw materials The individual raw material components are sampled and analysed in the laboratory for their ceramic properties and their mineralogical and chemical compositions. In the processing stage, the components are combined into the operating mass according to their ceramic properties, homogenised and stored. Forming The operating mass is pressed in extrusion presses under vacuum to form lumps, which are then pressed in turret or rotary table presses by means of plaster moulds to form roof tiles. Plain tiles are only extruded. Various parameters such as press vacuum, roof tile properties (moisture, plasticity and weight) are checked regularly. Excess operating mass and faulty pressings are returned in full to the mass circuit. Drying Drying serves as preparation of the plastic roofing tile for the subsequent firing process and takes place over 1–2 days at approx. 60–120 °C, depending on the model. Due to its shrinkage behaviour, the ceramic material reacts very sensitively and must therefore be dried under defined conditions. Various drying parameters and the residual moisture are constantly monitored. Dried roof tiles that have been sorted out (dry quarry) are returned to the production mass in the raw material preparation department. Colouring Engobes or glazes are applied to the dried roofing tiles as required. The density of the engobes/glazes and the application thickness are checked regularly. Any residues and the washing water are processed and returned to the raw material cycle. Firing The tiles are fired in tunnel kilns and bogie hearth furnaces at approx. 1000–1200 °C using natural gas. The firing time incl. the heating and cooling phase is approx. 1–2 days. The firing process gives the roof tiles their ceramic properties, which make them durable and long-lasting. Water-repellent finish In order to reduce the water absorption capacity, some roof tiles are hydrophobised on the surface in an immersion bath before being packed. Quality control The requisite ceramic quality properties according to EN 1304 and the product dimensions to be adhered to are regularly controlled internally in the factory's own production control and additionally monitored externally at least once a year. \nDeclared unit: \nThis Declaration refers to the manufacture of one square metre roofing tiles (40 kg/m²].", "lang": "en"}], "technologicalApplicability": [{"value": "Tondachziegel werden zum Eindecken von geneigten Dächern oder zur Verkleidung von Fassaden verwendet.", "lang": "de"}, {"value": "Clay roofing tiles are used for covering pitched roofs or for cladding facades.", "lang": "en"}], "referenceToTechnologyFlowDiagrammOrPicture": [{"shortDescription": [{"value": "Bautechnische Daten.jpg", "lang": "de"}], "type": "source data set", "refObjectId": "e4197c38-acfc-42e3-9d86-ff0a5c574a21", "uri": "../sources/e4197c38-acfc-42e3-9d86-ff0a5c574a21.xml"}]}}, "modellingAndValidation": {"LCIMethodAndAllocation": {"typeOfDataSet": "EPD", "referenceToLCAMethodDetails": [{"shortDescription": [{"value": "Dachziegel.pdf", "lang": "de"}], "type": "source data set", "refObjectId": "dc1688db-0c20-4532-b1bc-7c41ad93859f"}], "other": {"anies": [{"name": "subType", "value": "average dataset"}]}}, "dataSourcesTreatmentAndRepresentativeness": {"referenceToDataSource": [{"shortDescription": [{"value": "GaBi Database (all versions)", "lang": "de"}], "type": "source data set", "refObjectId": "28d74cc0-db8b-4d7e-bc44-5f6d56ce0c4a"}, {"shortDescription": [{"value": "GaBi database SP40 2020", "lang": "de"}], "type": "source data set", "refObjectId": "0115289e-52f0-4920-bc7e-57b1c96aec8d"}], "useAdviceForDataSet": [{"value": "Gültigkeitsbereich: \nDie Anwendung dieses Dokumentes ist auf Dachziegel beschränkt, die von Mitgliedsunternehmen des Bundesverbandes der Deutschen Ziegelindustrie e.V. hergestellt werden. Für diese Deklaration wurden von \n\n8 Mitgliedsunternehmen und insgesamt 20 Produktionsstandorten Daten aus dem Jahr 2020 zur Verfügung gestellt. Diese Mitglieder repräsentieren nach Anzahl rund 85 % der im Bundesverband zusammengeschlossenen Hersteller von Dachziegeln. Das Produktionsvolumen dieser Firmen liegt ­ nach Produktionsmenge- ­bei ca. 85 % des deutschen Marktes \nSystemgrenze: \nTyp der EPD: Wiege bis zum Werkstor - ­mit Optionen. Die Ökobilanz berücksichtigt die Rohstoffgewinnung, die Rohstofftransporte und die eigentliche Produktherstellung inklusive der Verpackungsmaterialien (Module A1 – A3). Der Transport zur Baustelle (Modul A4) sowie die Behandlung der Verpackungsmaterialien in Müllverbrennungsanlagen nach dem Einbau des Produktes (Modul A5) sind ebenfalls Teil der Systemgrenzen. Nach Ablauf der Nutzungsdauer wird das Produkt händisch rückgebaut (Modul C1). Nach dem Transport des rückgebauten Produktes (Modul C2) ist für rund 6 % der Dachziegel eine Deponierung auf einer Inertstoffdeponie vorgesehen (Modul C4), 94 \n\n% können weiterverwertet werden. Gutschriften infolge des Recyclings von Ziegelbruch sind in Modul D deklariert. Gutschriften für Strom und thermische Energie infolge der thermischen Verwertung der Verpackung innerhalb des Moduls A5 werden \n\nebenfalls in Modul D/1 berücksichtigt.", "lang": "de"}, {"value": "Scope: \nApplication of this document is restricted to roofing tiles manufactured by member companies of the Bundesverband der Deutschen Ziegelindustrie e.V. For this Declaration, \n\ndata from 2020 was made available by 8 member companies and a total of 20 production locations. These members represent around 85% of the manufacturers of roofing tiles united in the federal association. Depending on their respective production quantities, the production volume of these companies accounts for approx. 85% of the German market. \nSystem boundary: \nType of EPD: cradle to plant gate – with options. The Life Cycle Assessment takes into account the extraction of raw materials, the transport of raw materials and actual product manufacturing, including packaging materials (Modules A1–A3). Transport to the construction site (Module A4) and treatment of the packaging materials in the waste incineration plants following installation of the product (Module A5) are also part of the system boundaries. At the end of its useful life, the product is deconstructed by hand (Module C1). After transport of the dismantled product (Module C2), about 6% of the roofing tiles are to be disposed of in an inert waste landfill (Module C4), 94% can be recycled. Credits incurred by recycling firing waste are declared in Module D. Credits for electricity and thermal energy following thermal utilisation of packaging within Module A5 are also considered in Module D.", "lang": "en"}], "other": {"anies": [{"name": "referenceToOriginalEPD", "value": {"shortDescription": {"value": "Dachziegel (inklusive Zubehör).pdf", "defaultValue": "Dachziegel (inklusive Zubehör).pdf", "lstrings": [{"lang": "de", "value": "Dachziegel (inklusive Zubehör).pdf"}]}, "type": "source data set", "uuid": {"uuid": "a50dfa10-7b4b-4f23-ac9a-5e066c0eee2c"}, "refObjectId": "a50dfa10-7b4b-4f23-ac9a-5e066c0eee2c", "resourceURLs": ["https://oekobaudat.de/OEKOBAU.DAT/resource/sources/a50dfa10-7b4b-4f23-ac9a-5e066c0eee2c/Dachziegel_inklusive_Zubehoer__24182.pdf?version=00.04.000"]}}]}}, "validation": {"review": [{"referenceToNameOfReviewerAndInstitution": [{"shortDescription": [{"value": "Institut Bauen und Umwelt e. V.", "lang": "de"}], "type": "contact data set", "refObjectId": "d111dbec-b024-4be5-86c5-752d6eb2cf95", "uri": "../contacts/d111dbec-b024-4be5-86c5-752d6eb2cf95.xml"}], "type": "Accredited third party review"}]}, "complianceDeclarations": {"compliance": [{"referenceToComplianceSystem": {"shortDescription": [{"value": "DIN EN 15804+A2", "lang": "de"}], "type": "source data set", "refObjectId": "c0016b33-8cf7-415c-ac6e-deba0d21440d", "uri": "../sources/c0016b33-8cf7-415c-ac6e-deba0d21440d.xml"}}, {"referenceToComplianceSystem": {"shortDescription": [{"value": "ISO 14025", "lang": "de"}], "type": "source data set", "refObjectId": "4f2eb655-6e44-4874-a95a-e28f5442cd4d", "uri": "../sources/4f2eb655-6e44-4874-a95a-e28f5442cd4d.xml"}}]}}, "administrativeInformation": {"commissionerAndGoal": {"referenceToCommissioner": [{"shortDescription": [{"value": "Bundesverband der Deutschen Ziegelindustrie e.V.", "lang": "de"}], "type": "contact data set", "refObjectId": "44c3c786-9704-4e55-9729-ab211a1916fb", "uri": "../contacts/44c3c786-9704-4e55-9729-ab211a1916fb.xml"}]}, "dataGenerator": {"referenceToPersonOrEntityGeneratingTheDataSet": [{"shortDescription": [{"value": "Life Cycle Engineering Experts GmbH", "lang": "de"}], "type": "contact data set", "refObjectId": "2eed094a-ec91-42be-9e41-01ae55b495b9", "uri": "../contacts/2eed094a-ec91-42be-9e41-01ae55b495b9.xml"}]}, "dataEntryBy": {"timeStamp": 1636992092836, "referenceToDataSetFormat": [{"shortDescription": [{"value": "ILCD Format", "lang": "de"}], "type": "source data set", "refObjectId": "a97a0155-0234-4b87-b4ce-a45da52f2a40", "uri": "../sources/a97a0155-0234-4b87-b4ce-a45da52f2a40.xml"}, {"shortDescription": [{"value": "EPD-Datenformaterweiterungen v1.2", "lang": "de"}, {"value": "EPD Data Format Extensions v1.2", "lang": "en"}], "type": "source data set", "refObjectId": "a29449fd-aa2f-4de8-b5d7-4b06b43c6fde", "uri": "../sources/a29449fd-aa2f-4de8-b5d7-4b06b43c6fde.xml"}]}, "publicationAndOwnership": {"dataSetVersion": "00.01.000", "referenceToRegistrationAuthority": {"shortDescription": [{"value": "Institut Bauen und Umwelt e. V.", "lang": "de"}], "type": "contact data set", "refObjectId": "d111dbec-b024-4be5-86c5-752d6eb2cf95", "uri": "../contacts/d111dbec-b024-4be5-86c5-752d6eb2cf95.xml"}, "registrationNumber": "EPD-BDZ-20210268-IBG2-DE", "referenceToOwnershipOfDataSet": {"shortDescription": [{"value": "Bundesverband der Deutschen Ziegelindustrie e.V.", "lang": "de"}], "type": "contact data set", "refObjectId": "44c3c786-9704-4e55-9729-ab211a1916fb", "uri": "../contacts/44c3c786-9704-4e55-9729-ab211a1916fb.xml"}, "copyright": true, "licenseType": "Free of charge for all users and uses", "accessRestrictions": [{"value": "None", "lang": "en"}], "other": {"anies": [{"name": "referenceToPublisher", "value": {"shortDescription": [{"value": "Institut Bauen und Umwelt e. V.", "lang": "de"}], "type": "contact data set", "refObjectId": "d111dbec-b024-4be5-86c5-752d6eb2cf95", "uri": "../contacts/d111dbec-b024-4be5-86c5-752d6eb2cf95.xml"}}]}}}, "exchanges": {"exchange": [{"dataSetInternalID": 0, "referenceToFlowDataSet": {"shortDescription": [{"value": "Dachziegel (inklusive Zubehör) ()", "lang": "de"}], "type": "flow data set", "refObjectId": "4ad5e2ae-b68f-dd54-1b34-143dee9c5ec2", "uri": "../flows/4ad5e2ae-b68f-dd54-1b34-143dee9c5ec2.xml"}, "meanAmount": 1.0, "referencesToDataSource": {}, "referenceFlow": true, "resolvedFlowVersion": "00.01.000", "resultingflowAmount": 1.0, "flowProperties": [{"name": [{"lang": "en", "value": "Area"}, {"lang": "de", "value": "Fläche"}], "uuid": "93a60a56-a3c8-19da-a746-0800200c9a66", "referenceFlowProperty": true, "meanValue": 1.0, "referenceUnit": "qm", "unitGroupUUID": "c20a03d7-bd90-4569-bc94-66cfd364dfc8"}], "materialProperties": [{"name": "gross density", "value": "2020.0", "unit": "kg/m^3", "unitDescription": "kilograms per cubic metre"}, {"name": "conversion factor to 1 kg", "value": "40.0", "unit": "-", "unitDescription": "Without unit"}, {"name": "grammage", "value": "40.0", "unit": "kg/m^2", "unitDescription": "kilograms per square meter"}, {"name": "layer thickness", "value": "0.015", "unit": "m", "unitDescription": "meters"}], "typeOfFlow": "Product flow", "classification": {"classHierarchy": "Mineralische Baustoffe / Steine und Elemente / Dachziegel", "name": "OEKOBAU.DAT"}}, {"dataSetInternalID": 1, "referenceToFlowDataSet": {"shortDescription": [{"value": "Erneuerbare Primärenergie als Energieträger (PERE)", "lang": "de"}, {"value": "Renewable primary energy as energy carrier (PERE)", "lang": "en"}], "type": "flow data set", "refObjectId": "20f32be5-0398-4288-9b6d-accddd195317", "uri": "../flows/20f32be5-0398-4288-9b6d-accddd195317.xml"}, "exchange direction": "INPUT", "other": {"anies": [{"name": "referenceToUnitGroupDataSet", "value": {"shortDescription": [{"value": "MJ", "lang": "de"}], "type": "unit group data set", "refObjectId": "93a60a57-a3c8-11da-a746-0800200c9a66", "uri": "../unitgroups/93a60a57-a3c8-11da-a746-0800200c9a66.xml"}}, {"value": "35.55", "module": "A1-A3"}, {"value": "0.605", "module": "A4"}, {"value": "1.41", "module": "A5"}, {"value": "0", "module": "C1"}, {"value": "0.0505", "module": "C2"}, {"value": "0.158", "module": "C3"}, {"value": "0.0653", "module": "C4"}, {"value": "-2.47", "module": "D", "scenario": "S0"}, {"value": "-0.612", "module": "D", "scenario": "S1"}]}, "resolvedFlowVersion": "38.00.000", "flowProperties": [], "typeOfFlow": "Other flow", "classification": {"classHierarchy": "Quantities", "name": "GaBiCategories"}}, {"dataSetInternalID": 2, "referenceToFlowDataSet": {"shortDescription": [{"value": "Erneuerbare Primärenergie zur stofflichen Nutzung (PERM)", "lang": "de"}, {"value": "Renewable primary energy resources as material utilization (PERM)", "lang": "en"}], "type": "flow data set", "refObjectId": "fb3ec0de-548d-4508-aea5-00b73bf6f702", "uri": "../flows/fb3ec0de-548d-4508-aea5-00b73bf6f702.xml"}, "exchange direction": "INPUT", "other": {"anies": [{"name": "referenceToUnitGroupDataSet", "value": {"shortDescription": [{"value": "MJ", "lang": "de"}], "type": "unit group data set", "refObjectId": "93a60a57-a3c8-11da-a746-0800200c9a66", "uri": "../unitgroups/93a60a57-a3c8-11da-a746-0800200c9a66.xml"}}, {"value": "1.4", "module": "A1-A3"}, {"value": "0", "module": "A4"}, {"value": "-1.4", "module": "A5"}, {"value": "0", "module": "C1"}, {"value": "0", "module": "C2"}, {"value": "0", "module": "C3"}, {"value": "0", "module": "C4"}, {"value": "0", "module": "D", "scenario": "S0"}, {"value": "0", "module": "D", "scenario": "S1"}]}, "resolvedFlowVersion": "38.00.000", "flowProperties": [], "typeOfFlow": "Other flow", "classification": {"classHierarchy": "Quantities", "name": "GaBiCategories"}}, {"dataSetInternalID": 3, "referenceToFlowDataSet": {"shortDescription": [{"value": "Total erneuerbare Primärenergie (PERT)", "lang": "de"}, {"value": "Total use of renewable primary energy resources (PERT)", "lang": "en"}], "type": "flow data set", "refObjectId": "53f97275-fa8a-4cdd-9024-65936002acd0", "uri": "../flows/53f97275-fa8a-4cdd-9024-65936002acd0.xml"}, "exchange direction": "INPUT", "other": {"anies": [{"name": "referenceToUnitGroupDataSet", "value": {"shortDescription": [{"value": "MJ", "lang": "de"}], "type": "unit group data set", "refObjectId": "93a60a57-a3c8-11da-a746-0800200c9a66", "uri": "../unitgroups/93a60a57-a3c8-11da-a746-0800200c9a66.xml"}}, {"value": "36.95", "module": "A1-A3"}, {"value": "0.605", "module": "A4"}, {"value": "0.0126", "module": "A5"}, {"value": "0", "module": "C1"}, {"value": "0.0505", "module": "C2"}, {"value": "0.158", "module": "C3"}, {"value": "0.0653", "module": "C4"}, {"value": "-2.47", "module": "D", "scenario": "S0"}, {"value": "-0.612", "module": "D", "scenario": "S1"}]}, "resolvedFlowVersion": "38.00.000", "flowProperties": [], "typeOfFlow": "Other flow", "classification": {"classHierarchy": "Quantities / Environmental quantities / EPD EN 15804 / LCI indicators", "name": "GaBiCategories"}}, {"dataSetInternalID": 4, "referenceToFlowDataSet": {"shortDescription": [{"value": "Nicht-erneuerbare Primärenergie als Energieträger (PENRE)", "lang": "de"}, {"value": "Non renewable primary energy as energy carrier (PENRE)", "lang": "en"}], "type": "flow data set", "refObjectId": "ac857178-2b45-46ec-892a-a9a4332f0372", "uri": "../flows/ac857178-2b45-46ec-892a-a9a4332f0372.xml"}, "exchange direction": "INPUT", "other": {"anies": [{"name": "referenceToUnitGroupDataSet", "value": {"shortDescription": [{"value": "MJ", "lang": "de"}], "type": "unit group data set", "refObjectId": "93a60a57-a3c8-11da-a746-0800200c9a66", "uri": "../unitgroups/93a60a57-a3c8-11da-a746-0800200c9a66.xml"}}, {"value": "195.66", "module": "A1-A3"}, {"value": "10.4", "module": "A4"}, {"value": "0.0595", "module": "A5"}, {"value": "0", "module": "C1"}, {"value": "0.867", "module": "C2"}, {"value": "1.88", "module": "C3"}, {"value": "0.498", "module": "C4"}, {"value": "-79.6", "module": "D", "scenario": "S0"}, {"value": "-2.23", "module": "D", "scenario": "S1"}]}, "resolvedFlowVersion": "38.00.000", "flowProperties": [], "typeOfFlow": "Other flow", "classification": {"classHierarchy": "Quantities", "name": "GaBiCategories"}}, {"dataSetInternalID": 5, "referenceToFlowDataSet": {"shortDescription": [{"value": "Nicht-erneuerbare Primärenergie zur stofflichen Nutzung (PENRM)", "lang": "de"}, {"value": "Non renewable primary energy as material utilization (PENRM)", "lang": "en"}], "type": "flow data set", "refObjectId": "1421caa0-679d-4bf4-b282-0eb850ccae27", "uri": "../flows/1421caa0-679d-4bf4-b282-0eb850ccae27.xml"}, "exchange direction": "INPUT", "other": {"anies": [{"name": "referenceToUnitGroupDataSet", "value": {"shortDescription": [{"value": "MJ", "lang": "de"}], "type": "unit group data set", "refObjectId": "93a60a57-a3c8-11da-a746-0800200c9a66", "uri": "../unitgroups/93a60a57-a3c8-11da-a746-0800200c9a66.xml"}}, {"value": "0.88", "module": "A1-A3"}, {"value": "0", "module": "A4"}, {"value": "-0.88", "module": "A5"}, {"value": "0", "module": "C1"}, {"value": "0", "module": "C2"}, {"value": "0", "module": "C3"}, {"value": "0", "module": "C4"}, {"value": "0", "module": "D", "scenario": "S0"}, {"value": "0", "module": "D", "scenario": "S1"}]}, "resolvedFlowVersion": "38.00.000", "flowProperties": [], "typeOfFlow": "Other flow", "classification": {"classHierarchy": "Quantities", "name": "GaBiCategories"}}, {"dataSetInternalID": 6, "referenceToFlowDataSet": {"shortDescription": [{"value": "Total nicht erneuerbare Primärenergie (PENRT)", "lang": "de"}, {"value": "Total use of non renewable primary energy resources (PENRT)", "lang": "en"}], "type": "flow data set", "refObjectId": "06159210-646b-4c8d-8583-da9b3b95a6c1", "uri": "../flows/06159210-646b-4c8d-8583-da9b3b95a6c1.xml"}, "exchange direction": "INPUT", "other": {"anies": [{"name": "referenceToUnitGroupDataSet", "value": {"shortDescription": [{"value": "MJ", "lang": "de"}], "type": "unit group data set", "refObjectId": "93a60a57-a3c8-11da-a746-0800200c9a66", "uri": "../unitgroups/93a60a57-a3c8-11da-a746-0800200c9a66.xml"}}, {"value": "196.54", "module": "A1-A3"}, {"value": "10.4", "module": "A4"}, {"value": "-0.82", "module": "A5"}, {"value": "0", "module": "C1"}, {"value": "0.867", "module": "C2"}, {"value": "1.88", "module": "C3"}, {"value": "0.498", "module": "C4"}, {"value": "-79.6", "module": "D", "scenario": "S0"}, {"value": "-2.23", "module": "D", "scenario": "S1"}]}, "resolvedFlowVersion": "38.00.000", "flowProperties": [], "typeOfFlow": "Other flow", "classification": {"classHierarchy": "Quantities / Environmental quantities / EPD EN 15804 / LCI indicators", "name": "GaBiCategories"}}, {"dataSetInternalID": 7, "referenceToFlowDataSet": {"shortDescription": [{"value": "Einsatz von Sekundärstoffen (SM)", "lang": "de"}, {"value": "Use of secondary material (SM)", "lang": "en"}], "type": "flow data set", "refObjectId": "c6a1f35f-2d09-4f54-8dfb-97e502e1ce92", "uri": "../flows/c6a1f35f-2d09-4f54-8dfb-97e502e1ce92.xml"}, "exchange direction": "INPUT", "other": {"anies": [{"name": "referenceToUnitGroupDataSet", "value": {"shortDescription": [{"value": "kg", "lang": "de"}], "type": "unit group data set", "refObjectId": "ad38d542-3fe9-439d-9b95-2f5f7752acaf", "uri": "../unitgroups/ad38d542-3fe9-439d-9b95-2f5f7752acaf.xml"}}, {"value": "0.32", "module": "A1-A3"}, {"value": "0", "module": "A4"}, {"value": "0", "module": "A5"}, {"value": "0", "module": "C1"}, {"value": "0", "module": "C2"}, {"value": "0", "module": "C3"}, {"value": "0", "module": "C4"}, {"value": "37.5", "module": "D", "scenario": "S0"}, {"value": "0", "module": "D", "scenario": "S1"}]}, "resolvedFlowVersion": "38.00.000", "flowProperties": [], "typeOfFlow": "Other flow", "classification": {"classHierarchy": "Quantities / Environmental quantities / EPD EN 15804 / LCI indicators", "name": "GaBiCategories"}}, {"dataSetInternalID": 8, "referenceToFlowDataSet": {"shortDescription": [{"value": "Erneuerbare Sekundärbrennstoffe (RSF)", "lang": "de"}, {"value": "Use of renewable secondary fuels (RSF)", "lang": "en"}], "type": "flow data set", "refObjectId": "64333088-a55f-4aa2-9a31-c10b07816787", "uri": "../flows/64333088-a55f-4aa2-9a31-c10b07816787.xml"}, "exchange direction": "INPUT", "other": {"anies": [{"name": "referenceToUnitGroupDataSet", "value": {"shortDescription": [{"value": "MJ", "lang": "de"}], "type": "unit group data set", "refObjectId": "93a60a57-a3c8-11da-a746-0800200c9a66", "uri": "../unitgroups/93a60a57-a3c8-11da-a746-0800200c9a66.xml"}}, {"value": "0", "module": "A1-A3"}, {"value": "0", "module": "A4"}, {"value": "0", "module": "A5"}, {"value": "0", "module": "C1"}, {"value": "0", "module": "C2"}, {"value": "0", "module": "C3"}, {"value": "0", "module": "C4"}, {"value": "0", "module": "D", "scenario": "S0"}, {"value": "0", "module": "D", "scenario": "S1"}]}, "resolvedFlowVersion": "38.00.000", "flowProperties": [], "typeOfFlow": "Other flow", "classification": {"classHierarchy": "Quantities / Environmental quantities / EPD EN 15804 / LCI indicators", "name": "GaBiCategories"}}, {"dataSetInternalID": 9, "referenceToFlowDataSet": {"shortDescription": [{"value": "Nicht erneuerbare Sekundärbrennstoffe (NRSF)", "lang": "de"}, {"value": "Use of non renewable secondary fuels (NRSF)", "lang": "en"}], "type": "flow data set", "refObjectId": "89def144-d39a-4287-b86f-efde453ddcb2", "uri": "../flows/89def144-d39a-4287-b86f-efde453ddcb2.xml"}, "exchange direction": "INPUT", "other": {"anies": [{"name": "referenceToUnitGroupDataSet", "value": {"shortDescription": [{"value": "MJ", "lang": "de"}], "type": "unit group data set", "refObjectId": "93a60a57-a3c8-11da-a746-0800200c9a66", "uri": "../unitgroups/93a60a57-a3c8-11da-a746-0800200c9a66.xml"}}, {"value": "0", "module": "A1-A3"}, {"value": "0", "module": "A4"}, {"value": "0", "module": "A5"}, {"value": "0", "module": "C1"}, {"value": "0", "module": "C2"}, {"value": "0", "module": "C3"}, {"value": "0", "module": "C4"}, {"value": "0", "module": "D", "scenario": "S0"}, {"value": "0", "module": "D", "scenario": "S1"}]}, "resolvedFlowVersion": "38.00.000", "flowProperties": [], "typeOfFlow": "Other flow", "classification": {"classHierarchy": "Quantities / Environmental quantities / EPD EN 15804 / LCI indicators", "name": "GaBiCategories"}}, {"dataSetInternalID": 10, "referenceToFlowDataSet": {"shortDescription": [{"value": "Einsatz von Süßwasserressourcen (FW)", "lang": "de"}, {"value": "Use of net fresh water (FW)", "lang": "en"}], "type": "flow data set", "refObjectId": "3cf952c8-f3a4-461d-8c96-96456ca62246", "uri": "../flows/3cf952c8-f3a4-461d-8c96-96456ca62246.xml"}, "exchange direction": "INPUT", "other": {"anies": [{"name": "referenceToUnitGroupDataSet", "value": {"shortDescription": [{"value": "m^3", "lang": "de"}], "type": "unit group data set", "refObjectId": "cd950537-0a98-4044-9ba7-9f9a68d0a504", "uri": "../unitgroups/cd950537-0a98-4044-9ba7-9f9a68d0a504.xml"}}, {"value": "0.0216", "module": "A1-A3"}, {"value": "0.000542", "module": "A4"}, {"value": "0.000658", "module": "A5"}, {"value": "0", "module": "C1"}, {"value": "4.52E-05", "module": "C2"}, {"value": "0.000493", "module": "C3"}, {"value": "0.000125", "module": "C4"}, {"value": "-0.00177", "module": "D", "scenario": "S0"}, {"value": "-0.000334", "module": "D", "scenario": "S1"}]}, "resolvedFlowVersion": "38.00.000", "flowProperties": [], "typeOfFlow": "Other flow", "classification": {"classHierarchy": "Quantities / Environmental quantities / EPD EN 15804 / LCI indicators", "name": "GaBiCategories"}}, {"dataSetInternalID": 11, "referenceToFlowDataSet": {"shortDescription": [{"value": "Gefährlicher Abfall zur Deponie (HWD)", "lang": "de"}, {"value": "Hazardous waste disposed (HWD)", "lang": "en"}], "type": "flow data set", "refObjectId": "430f9e0f-59b2-46a0-8e0d-55e0e84948fc", "uri": "../flows/430f9e0f-59b2-46a0-8e0d-55e0e84948fc.xml"}, "exchange direction": "OUTPUT", "other": {"anies": [{"name": "referenceToUnitGroupDataSet", "value": {"shortDescription": [{"value": "kg", "lang": "de"}], "type": "unit group data set", "refObjectId": "ad38d542-3fe9-439d-9b95-2f5f7752acaf", "uri": "../unitgroups/ad38d542-3fe9-439d-9b95-2f5f7752acaf.xml"}}, {"value": "3.364E-07", "module": "A1-A3"}, {"value": "3.89E-07", "module": "A4"}, {"value": "7.88E-11", "module": "A5"}, {"value": "0", "module": "C1"}, {"value": "3.24E-08", "module": "C2"}, {"value": "3.96E-08", "module": "C3"}, {"value": "7.59E-09", "module": "C4"}, {"value": "-1.56E-07", "module": "D", "scenario": "S0"}, {"value": "-1.2E-09", "module": "D", "scenario": "S1"}]}, "resolvedFlowVersion": "38.00.000", "flowProperties": [], "typeOfFlow": "Other flow", "classification": {"classHierarchy": "Quantities / Environmental quantities / EPD EN 15804 / LCI indicators", "name": "GaBiCategories"}}, {"dataSetInternalID": 12, "referenceToFlowDataSet": {"shortDescription": [{"value": "Entsorgter nicht gefährlicher Abfall (NHWD)", "lang": "de"}, {"value": "Non hazardous waste disposed (NHWD)", "lang": "en"}], "type": "flow data set", "refObjectId": "b29ef66b-e286-4afa-949f-62f1a7b4d7fa", "uri": "../flows/b29ef66b-e286-4afa-949f-62f1a7b4d7fa.xml"}, "exchange direction": "OUTPUT", "other": {"anies": [{"name": "referenceToUnitGroupDataSet", "value": {"shortDescription": [{"value": "kg", "lang": "de"}], "type": "unit group data set", "refObjectId": "ad38d542-3fe9-439d-9b95-2f5f7752acaf", "uri": "../unitgroups/ad38d542-3fe9-439d-9b95-2f5f7752acaf.xml"}}, {"value": "0.111353", "module": "A1-A3"}, {"value": "0.00183", "module": "A4"}, {"value": "0.00319", "module": "A5"}, {"value": "0", "module": "C1"}, {"value": "0.000152", "module": "C2"}, {"value": "0.000567", "module": "C3"}, {"value": "2.5", "module": "C4"}, {"value": "-0.0222", "module": "D", "scenario": "S0"}, {"value": "-0.0011", "module": "D", "scenario": "S1"}]}, "resolvedFlowVersion": "38.00.000", "flowProperties": [], "typeOfFlow": "Other flow", "classification": {"classHierarchy": "Quantities / Environmental quantities / EPD EN 15804 / LCI indicators", "name": "GaBiCategories"}}, {"dataSetInternalID": 13, "referenceToFlowDataSet": {"shortDescription": [{"value": "Entsorgter radioaktiver Abfall (RWD)", "lang": "de"}, {"value": "Radioactive waste disposed (RWD)", "lang": "en"}], "type": "flow data set", "refObjectId": "3449546e-52ad-4b39-b809-9fb77cea8ff6", "uri": "../flows/3449546e-52ad-4b39-b809-9fb77cea8ff6.xml"}, "exchange direction": "OUTPUT", "other": {"anies": [{"name": "referenceToUnitGroupDataSet", "value": {"shortDescription": [{"value": "kg", "lang": "de"}], "type": "unit group data set", "refObjectId": "ad38d542-3fe9-439d-9b95-2f5f7752acaf", "uri": "../unitgroups/ad38d542-3fe9-439d-9b95-2f5f7752acaf.xml"}}, {"value": "0.00305218", "module": "A1-A3"}, {"value": "1.09E-05", "module": "A4"}, {"value": "2.33E-06", "module": "A5"}, {"value": "0", "module": "C1"}, {"value": "9.12E-07", "module": "C2"}, {"value": "1.51E-05", "module": "C3"}, {"value": "5.58E-06", "module": "C4"}, {"value": "-0.000347", "module": "D", "scenario": "S0"}, {"value": "-8.88E-05", "module": "D", "scenario": "S1"}]}, "resolvedFlowVersion": "38.00.000", "flowProperties": [], "typeOfFlow": "Other flow", "classification": {"classHierarchy": "Quantities / Environmental quantities / EPD EN 15804 / LCI indicators", "name": "GaBiCategories"}}, {"dataSetInternalID": 14, "referenceToFlowDataSet": {"shortDescription": [{"value": "Komponenten für die Wiederverwendung (CRU)", "lang": "de"}, {"value": "Components for re-use (CRU)", "lang": "en"}], "type": "flow data set", "refObjectId": "a2b32f97-3fc7-4af2-b209-525bc6426f33", "uri": "../flows/a2b32f97-3fc7-4af2-b209-525bc6426f33.xml"}, "exchange direction": "OUTPUT", "other": {"anies": [{"name": "referenceToUnitGroupDataSet", "value": {"shortDescription": [{"value": "kg", "lang": "de"}], "type": "unit group data set", "refObjectId": "ad38d542-3fe9-439d-9b95-2f5f7752acaf", "uri": "../unitgroups/ad38d542-3fe9-439d-9b95-2f5f7752acaf.xml"}}, {"value": "0", "module": "A1-A3"}, {"value": "0", "module": "A4"}, {"value": "0", "module": "A5"}, {"value": "0", "module": "C1"}, {"value": "0", "module": "C2"}, {"value": "0", "module": "C3"}, {"value": "0", "module": "C4"}, {"value": "0", "module": "D", "scenario": "S0"}, {"value": "0", "module": "D", "scenario": "S1"}]}, "resolvedFlowVersion": "38.00.000", "flowProperties": [], "typeOfFlow": "Other flow", "classification": {"classHierarchy": "Quantities / Environmental quantities / EPD EN 15804 / LCI indicators", "name": "GaBiCategories"}}, {"dataSetInternalID": 15, "referenceToFlowDataSet": {"shortDescription": [{"value": "Stoffe zum Recycling (MFR)", "lang": "de"}, {"value": "Materials for recycling (MFR)", "lang": "en"}], "type": "flow data set", "refObjectId": "d7fe48a5-4103-49c8-9aae-b0b5dfdbd6ae", "uri": "../flows/d7fe48a5-4103-49c8-9aae-b0b5dfdbd6ae.xml"}, "exchange direction": "OUTPUT", "other": {"anies": [{"name": "referenceToUnitGroupDataSet", "value": {"shortDescription": [{"value": "kg", "lang": "de"}], "type": "unit group data set", "refObjectId": "ad38d542-3fe9-439d-9b95-2f5f7752acaf", "uri": "../unitgroups/ad38d542-3fe9-439d-9b95-2f5f7752acaf.xml"}}, {"value": "0", "module": "A1-A3"}, {"value": "0", "module": "A4"}, {"value": "0", "module": "A5"}, {"value": "0", "module": "C1"}, {"value": "0", "module": "C2"}, {"value": "40", "module": "C3"}, {"value": "0", "module": "C4"}, {"value": "0", "module": "D", "scenario": "S0"}, {"value": "0", "module": "D", "scenario": "S1"}]}, "resolvedFlowVersion": "38.00.000", "flowProperties": [], "typeOfFlow": "Other flow", "classification": {"classHierarchy": "Quantities / Environmental quantities / EPD EN 15804 / LCI indicators", "name": "GaBiCategories"}}, {"dataSetInternalID": 16, "referenceToFlowDataSet": {"shortDescription": [{"value": "Stoffe für die Energierückgewinnung (MER)", "lang": "de"}, {"value": "Materials for energy recovery (MER)", "lang": "en"}], "type": "flow data set", "refObjectId": "59a9181c-3aaf-46ee-8b13-2b3723b6e447", "uri": "../flows/59a9181c-3aaf-46ee-8b13-2b3723b6e447.xml"}, "exchange direction": "OUTPUT", "other": {"anies": [{"name": "referenceToUnitGroupDataSet", "value": {"shortDescription": [{"value": "kg", "lang": "de"}], "type": "unit group data set", "refObjectId": "ad38d542-3fe9-439d-9b95-2f5f7752acaf", "uri": "../unitgroups/ad38d542-3fe9-439d-9b95-2f5f7752acaf.xml"}}, {"value": "0", "module": "A1-A3"}, {"value": "0", "module": "A4"}, {"value": "0", "module": "A5"}, {"value": "0", "module": "C1"}, {"value": "0", "module": "C2"}, {"value": "0", "module": "C3"}, {"value": "0", "module": "C4"}, {"value": "0", "module": "D", "scenario": "S0"}, {"value": "0", "module": "D", "scenario": "S1"}]}, "resolvedFlowVersion": "38.00.000", "flowProperties": [], "typeOfFlow": "Other flow", "classification": {"classHierarchy": "Quantities / Environmental quantities / EPD EN 15804 / LCI indicators", "name": "GaBiCategories"}}, {"dataSetInternalID": 17, "referenceToFlowDataSet": {"shortDescription": [{"value": "Exportierte elektrische Energie (EEE)", "lang": "de"}, {"value": "Exported electrical energy (EEE)", "lang": "en"}], "type": "flow data set", "refObjectId": "4da0c987-2b76-40d6-9e9e-82a017aaaf29", "uri": "../flows/4da0c987-2b76-40d6-9e9e-82a017aaaf29.xml"}, "exchange direction": "OUTPUT", "other": {"anies": [{"name": "referenceToUnitGroupDataSet", "value": {"shortDescription": [{"value": "MJ", "lang": "de"}], "type": "unit group data set", "refObjectId": "93a60a57-a3c8-11da-a746-0800200c9a66", "uri": "../unitgroups/93a60a57-a3c8-11da-a746-0800200c9a66.xml"}}, {"value": "0", "module": "A1-A3"}, {"value": "0", "module": "A4"}, {"value": "0.448", "module": "A5"}, {"value": "0", "module": "C1"}, {"value": "0", "module": "C2"}, {"value": "0", "module": "C3"}, {"value": "0", "module": "C4"}, {"value": "0", "module": "D", "scenario": "S0"}, {"value": "0", "module": "D", "scenario": "S1"}]}, "resolvedFlowVersion": "38.00.000", "flowProperties": [], "typeOfFlow": "Other flow", "classification": {"classHierarchy": "Quantities / Environmental quantities / EPD EN 15804 / LCI indicators", "name": "GaBiCategories"}}, {"dataSetInternalID": 18, "referenceToFlowDataSet": {"shortDescription": [{"value": "Exportierte thermische Energie (EET)", "lang": "de"}, {"value": "Exported thermal energy (EET)", "lang": "en"}], "type": "flow data set", "refObjectId": "98daf38a-7a79-46d3-9a37-2b7bd0955810", "uri": "../flows/98daf38a-7a79-46d3-9a37-2b7bd0955810.xml"}, "exchange direction": "OUTPUT", "other": {"anies": [{"name": "referenceToUnitGroupDataSet", "value": {"shortDescription": [{"value": "MJ", "lang": "de"}], "type": "unit group data set", "refObjectId": "93a60a57-a3c8-11da-a746-0800200c9a66", "uri": "../unitgroups/93a60a57-a3c8-11da-a746-0800200c9a66.xml"}}, {"value": "0", "module": "A1-A3"}, {"value": "0", "module": "A4"}, {"value": "0.886", "module": "A5"}, {"value": "0", "module": "C1"}, {"value": "0", "module": "C2"}, {"value": "0", "module": "C3"}, {"value": "0", "module": "C4"}, {"value": "0", "module": "D", "scenario": "S0"}, {"value": "0", "module": "D", "scenario": "S1"}]}, "resolvedFlowVersion": "38.00.000", "flowProperties": [], "typeOfFlow": "Other flow", "classification": {"classHierarchy": "Quantities / Environmental quantities / EPD EN 15804 / LCI indicators", "name": "GaBiCategories"}}]}, "LCIAResults": {"LCIAResult": [{"referenceToLCIAMethodDataSet": {"shortDescription": [{"value": "Globales Erwärmungspotenzial total (GWP-total)", "lang": "de"}, {"value": "Global Warming Potential total (GWP-total)", "lang": "en"}], "type": "LCIA method data set", "refObjectId": "6a37f984-a4b3-458a-a20a-64418c145fa2", "uri": "../lciamethods/6a37f984-a4b3-458a-a20a-64418c145fa2.xml"}, "other": {"anies": [{"name": "referenceToUnitGroupDataSet", "value": {"shortDescription": [{"value": "kg CO_(2)-Äq.", "lang": "de"}], "type": "unit group data set", "refObjectId": "1ebf3012-d0db-4de2-aefd-ef30cedb0be1", "uri": "../unitgroups/1ebf3012-d0db-4de2-aefd-ef30cedb0be1.xml"}}, {"value": "12.329", "module": "A1-A3"}, {"value": "0.787", "module": "A4"}, {"value": "0.261", "module": "A5"}, {"value": "0", "module": "C1"}, {"value": "0.0656", "module": "C2"}, {"value": "0.1", "module": "C3"}, {"value": "0.041", "module": "C4"}, {"value": "-6.06", "module": "D", "scenario": "S0"}, {"value": "-0.158", "module": "D", "scenario": "S1"}]}}, {"referenceToLCIAMethodDataSet": {"shortDescription": [{"value": "Globales Erwärmungspotenzial fossil (GWP-fossil)", "lang": "de"}, {"value": "Global Warming Potential fossil fuels (GWP-fossil)", "lang": "en"}], "type": "LCIA method data set", "refObjectId": "5f635281-343e-44fb-83df-1971b155e6b6", "uri": "../lciamethods/5f635281-343e-44fb-83df-1971b155e6b6.xml"}, "other": {"anies": [{"name": "referenceToUnitGroupDataSet", "value": {"shortDescription": [{"value": "kg CO_(2)-Äq.", "lang": "de"}], "type": "unit group data set", "refObjectId": "1ebf3012-d0db-4de2-aefd-ef30cedb0be1", "uri": "../unitgroups/1ebf3012-d0db-4de2-aefd-ef30cedb0be1.xml"}}, {"value": "12.427", "module": "A1-A3"}, {"value": "0.783", "module": "A4"}, {"value": "0.138", "module": "A5"}, {"value": "0", "module": "C1"}, {"value": "0.0653", "module": "C2"}, {"value": "0.0998", "module": "C3"}, {"value": "0.038", "module": "C4"}, {"value": "-6.04", "module": "D", "scenario": "S0"}, {"value": "-0.157", "module": "D", "scenario": "S1"}]}}, {"referenceToLCIAMethodDataSet": {"shortDescription": [{"value": "Globales Erwärmungspotenzial biogen (GWP-biogenic)", "lang": "de"}, {"value": "Global Warming Potential biogenic (GWP-biogenic)", "lang": "en"}], "type": "LCIA method data set", "refObjectId": "2356e1ab-0185-4db5-86e5-16de51c7485c", "uri": "../lciamethods/2356e1ab-0185-4db5-86e5-16de51c7485c.xml"}, "other": {"anies": [{"name": "referenceToUnitGroupDataSet", "value": {"shortDescription": [{"value": "kg CO_(2)-Äq.", "lang": "de"}], "type": "unit group data set", "refObjectId": "1ebf3012-d0db-4de2-aefd-ef30cedb0be1", "uri": "../unitgroups/1ebf3012-d0db-4de2-aefd-ef30cedb0be1.xml"}}, {"value": "-0.1077783", "module": "A1-A3"}, {"value": "0.000315", "module": "A4"}, {"value": "0.123", "module": "A5"}, {"value": "0", "module": "C1"}, {"value": "2.62E-05", "module": "C2"}, {"value": "0.000191", "module": "C3"}, {"value": "0.00301", "module": "C4"}, {"value": "-0.0129", "module": "D", "scenario": "S0"}, {"value": "-0.000687", "module": "D", "scenario": "S1"}]}}, {"referenceToLCIAMethodDataSet": {"shortDescription": [{"value": "Globales Erwärmungspotenzial luluc (GWP-luluc)", "lang": "de"}, {"value": "Global Warming Potential luluc (GWP-luluc)", "lang": "en"}], "type": "LCIA method data set", "refObjectId": "4331bbdb-978a-490d-8707-eeb047f01a55", "uri": "../lciamethods/4331bbdb-978a-490d-8707-eeb047f01a55.xml"}, "other": {"anies": [{"name": "referenceToUnitGroupDataSet", "value": {"shortDescription": [{"value": "kg CO_(2)-Äq.", "lang": "de"}], "type": "unit group data set", "refObjectId": "1ebf3012-d0db-4de2-aefd-ef30cedb0be1", "uri": "../unitgroups/1ebf3012-d0db-4de2-aefd-ef30cedb0be1.xml"}}, {"value": "0.008034", "module": "A1-A3"}, {"value": "0.00328", "module": "A4"}, {"value": "4.52E-06", "module": "A5"}, {"value": "0", "module": "C1"}, {"value": "0.000273", "module": "C2"}, {"value": "0.000368", "module": "C3"}, {"value": "0.000109", "module": "C4"}, {"value": "-0.0021", "module": "D", "scenario": "S0"}, {"value": "-0.000218", "module": "D", "scenario": "S1"}]}}, {"referenceToLCIAMethodDataSet": {"shortDescription": [{"value": "Abbau Potential der stratosphärischen Ozonschicht (ODP)", "lang": "de"}, {"value": "Depletion potential of the stratospheric ozone layer (ODP)", "lang": "en"}], "type": "LCIA method data set", "refObjectId": "b5c629d6-def3-11e6-bf01-fe55135034f3", "uri": "../lciamethods/b5c629d6-def3-11e6-bf01-fe55135034f3.xml"}, "other": {"anies": [{"name": "referenceToUnitGroupDataSet", "value": {"shortDescription": [{"value": "kg CFC11-Äq.", "lang": "de"}], "type": "unit group data set", "refObjectId": "d9e957c9-7309-4474-bf3a-7777df6c4e5b", "uri": "../unitgroups/d9e957c9-7309-4474-bf3a-7777df6c4e5b.xml"}}, {"value": "1.0602433E-12", "module": "A1-A3"}, {"value": "1.92E-16", "module": "A4"}, {"value": "4.97E-17", "module": "A5"}, {"value": "0", "module": "C1"}, {"value": "1.6E-17", "module": "C2"}, {"value": "4.25E-16", "module": "C3"}, {"value": "1.42E-16", "module": "C4"}, {"value": "-9.48E-15", "module": "D", "scenario": "S0"}, {"value": "-2.61E-15", "module": "D", "scenario": "S1"}]}}, {"referenceToLCIAMethodDataSet": {"shortDescription": [{"value": "Versauerungspotenzial von Boden und Wasser (AP)", "lang": "de"}, {"value": "Acidification potential of land and water (AP)", "lang": "en"}], "type": "LCIA method data set", "refObjectId": "b5c611c6-def3-11e6-bf01-fe55135034f3", "uri": "../lciamethods/b5c611c6-def3-11e6-bf01-fe55135034f3.xml"}, "other": {"anies": [{"name": "referenceToUnitGroupDataSet", "value": {"shortDescription": [{"value": "mol H^(+)-Äq.", "lang": "de"}], "type": "unit group data set", "refObjectId": "42e089ac-92bf-4bf2-8ca1-5fc40d18f2ed", "uri": "../unitgroups/42e089ac-92bf-4bf2-8ca1-5fc40d18f2ed.xml"}}, {"value": "0.012783", "module": "A1-A3"}, {"value": "0.000727", "module": "A4"}, {"value": "5.45E-05", "module": "A5"}, {"value": "0", "module": "C1"}, {"value": "6.06E-05", "module": "C2"}, {"value": "0.000938", "module": "C3"}, {"value": "0.000272", "module": "C4"}, {"value": "-0.00935", "module": "D", "scenario": "S0"}, {"value": "-0.000178", "module": "D", "scenario": "S1"}]}}, {"referenceToLCIAMethodDataSet": {"shortDescription": [{"value": "Eutrophierungspotenzial Süßwasser (EP-freshwater)", "lang": "de"}, {"value": "Eutrophication potential aquatic freshwater (EP-freshwater)", "lang": "en"}], "type": "LCIA method data set", "refObjectId": "b53ec18f-7377-4ad3-86eb-cc3f4f276b2b", "uri": "../lciamethods/b53ec18f-7377-4ad3-86eb-cc3f4f276b2b.xml"}, "other": {"anies": [{"name": "referenceToUnitGroupDataSet", "value": {"shortDescription": [{"value": "kg PO_(4)-Äq.", "lang": "de"}], "type": "unit group data set", "refObjectId": "0429039d-a61d-4590-ba67-aa4a20a810a1", "uri": "../unitgroups/0429039d-a61d-4590-ba67-aa4a20a810a1.xml"}}, {"value": "1.7093E-05", "module": "A1-A3"}, {"value": "1.7E-06", "module": "A4"}, {"value": "8.42E-09", "module": "A5"}, {"value": "0", "module": "C1"}, {"value": "1.42E-07", "module": "C2"}, {"value": "2.39E-07", "module": "C3"}, {"value": "6.54E-08", "module": "C4"}, {"value": "-3.28E-06", "module": "D", "scenario": "S0"}, {"value": "-3.56E-07", "module": "D", "scenario": "S1"}]}}, {"referenceToLCIAMethodDataSet": {"shortDescription": [{"value": "Eutrophierungspotenzial Salzwasser (EP-marine)", "lang": "de"}, {"value": "Eutrophication potential aquatic marine (EP-marine)", "lang": "en"}], "type": "LCIA method data set", "refObjectId": "b5c619fa-def3-11e6-bf01-fe55135034f3", "uri": "../lciamethods/b5c619fa-def3-11e6-bf01-fe55135034f3.xml"}, "other": {"anies": [{"name": "referenceToUnitGroupDataSet", "value": {"shortDescription": [{"value": "kg N-Äq.", "lang": "de"}], "type": "unit group data set", "refObjectId": "d05bb823-ecdf-4686-8c40-bf1d9257859f", "uri": "../unitgroups/d05bb823-ecdf-4686-8c40-bf1d9257859f.xml"}}, {"value": "0.004588", "module": "A1-A3"}, {"value": "0.000226", "module": "A4"}, {"value": "1.66E-05", "module": "A5"}, {"value": "0", "module": "C1"}, {"value": "1.88E-05", "module": "C2"}, {"value": "0.000462", "module": "C3"}, {"value": "7E-05", "module": "C4"}, {"value": "-0.00378", "module": "D", "scenario": "S0"}, {"value": "-5.75E-05", "module": "D", "scenario": "S1"}]}}, {"referenceToLCIAMethodDataSet": {"shortDescription": [{"value": "Eutrophierungspotenzial Land (EP-terrestrial)", "lang": "de"}, {"value": "Eutrophication potential terrestrial (EP-terrestrial)", "lang": "en"}], "type": "LCIA method data set", "refObjectId": "b5c614d2-def3-11e6-bf01-fe55135034f3", "uri": "../lciamethods/b5c614d2-def3-11e6-bf01-fe55135034f3.xml"}, "other": {"anies": [{"name": "referenceToUnitGroupDataSet", "value": {"shortDescription": [{"value": "mol N-Äq.", "lang": "de"}], "type": "unit group data set", "refObjectId": "71b4d617-0ec9-4d3f-b65e-e438940c2401", "uri": "../unitgroups/71b4d617-0ec9-4d3f-b65e-e438940c2401.xml"}}, {"value": "0.04936", "module": "A1-A3"}, {"value": "0.00274", "module": "A4"}, {"value": "0.000251", "module": "A5"}, {"value": "0", "module": "C1"}, {"value": "0.000229", "module": "C2"}, {"value": "0.00508", "module": "C3"}, {"value": "0.00077", "module": "C4"}, {"value": "-0.0417", "module": "D", "scenario": "S0"}, {"value": "-0.000612", "module": "D", "scenario": "S1"}]}}, {"referenceToLCIAMethodDataSet": {"shortDescription": [{"value": "Bildungspotential für troposphärisches Ozon (POCP)", "lang": "de"}, {"value": "Formation potential of tropospheric ozone photochemical oxidants (POCP)", "lang": "en"}], "type": "LCIA method data set", "refObjectId": "b5c610fe-def3-11e6-bf01-fe55135034f3", "uri": "../lciamethods/b5c610fe-def3-11e6-bf01-fe55135034f3.xml"}, "other": {"anies": [{"name": "referenceToUnitGroupDataSet", "value": {"shortDescription": [{"value": "kg NMVOC-Äq.", "lang": "de"}], "type": "unit group data set", "refObjectId": "d27c25f8-fbc1-44c6-b47b-4adbae4199c6", "uri": "../unitgroups/d27c25f8-fbc1-44c6-b47b-4adbae4199c6.xml"}}, {"value": "0.012964", "module": "A1-A3"}, {"value": "0.000598", "module": "A4"}, {"value": "4.43E-05", "module": "A5"}, {"value": "0", "module": "C1"}, {"value": "4.98E-05", "module": "C2"}, {"value": "0.00134", "module": "C3"}, {"value": "0.000212", "module": "C4"}, {"value": "-0.011", "module": "D", "scenario": "S0"}, {"value": "-0.000153", "module": "D", "scenario": "S1"}]}}, {"referenceToLCIAMethodDataSet": {"shortDescription": [{"value": "Potenzial für den abiotischen Abbau nicht fossiler Ressourcen (ADPE)", "lang": "de"}, {"value": "Abiotic depletion potential for non fossil resources (ADPE)", "lang": "en"}], "type": "LCIA method data set", "refObjectId": "b2ad6494-c78d-11e6-9d9d-cec0c932ce01", "uri": "../lciamethods/b2ad6494-c78d-11e6-9d9d-cec0c932ce01.xml"}, "other": {"anies": [{"name": "referenceToUnitGroupDataSet", "value": {"shortDescription": [{"value": "kg Sb-Äq.", "lang": "de"}], "type": "unit group data set", "refObjectId": "54ccd2d9-a32a-4fc2-923d-f2c8c93e89d4", "uri": "../unitgroups/54ccd2d9-a32a-4fc2-923d-f2c8c93e89d4.xml"}}, {"value": "1.78601E-06", "module": "A1-A3"}, {"value": "6.5E-08", "module": "A4"}, {"value": "7.18E-10", "module": "A5"}, {"value": "0", "module": "C1"}, {"value": "5.42E-09", "module": "C2"}, {"value": "1.1E-07", "module": "C3"}, {"value": "3.42E-09", "module": "C4"}, {"value": "-3.17E-07", "module": "D", "scenario": "S0"}, {"value": "-3.62E-08", "module": "D", "scenario": "S1"}]}}, {"referenceToLCIAMethodDataSet": {"shortDescription": [{"value": "Potenzial für den abiotischen Abbau fossiler Brennstoffe (ADPF)", "lang": "de"}, {"value": "Abiotic depletion potential for fossil resources (ADPF)", "lang": "en"}], "type": "LCIA method data set", "refObjectId": "b2ad6110-c78d-11e6-9d9d-cec0c932ce01", "uri": "../lciamethods/b2ad6110-c78d-11e6-9d9d-cec0c932ce01.xml"}, "other": {"anies": [{"name": "referenceToUnitGroupDataSet", "value": {"shortDescription": [{"value": "MJ", "lang": "de"}], "type": "unit group data set", "refObjectId": "93a60a57-a3c8-11da-a746-0800200c9a66", "uri": "../unitgroups/93a60a57-a3c8-11da-a746-0800200c9a66.xml"}}, {"value": "195.66", "module": "A1-A3"}, {"value": "10.4", "module": "A4"}, {"value": "0.0595", "module": "A5"}, {"value": "0", "module": "C1"}, {"value": "0.867", "module": "C2"}, {"value": "1.88", "module": "C3"}, {"value": "0.498", "module": "C4"}, {"value": "-79.6", "module": "D", "scenario": "S0"}, {"value": "-2.23", "module": "D", "scenario": "S1"}]}}, {"referenceToLCIAMethodDataSet": {"shortDescription": [{"value": "Wassernutzung (WDP)", "lang": "de"}, {"value": "Water use (WDP)", "lang": "en"}], "type": "LCIA method data set", "refObjectId": "b2ad66ce-c78d-11e6-9d9d-cec0c932ce01", "uri": "../lciamethods/b2ad66ce-c78d-11e6-9d9d-cec0c932ce01.xml"}, "other": {"anies": [{"name": "referenceToUnitGroupDataSet", "value": {"shortDescription": [{"value": "m^(3) Welt-Äq. entzogen", "lang": "de"}], "type": "unit group data set", "refObjectId": "6ae2df01-888e-46c8-b17d-49fa3869b476", "uri": "../unitgroups/6ae2df01-888e-46c8-b17d-49fa3869b476.xml"}}, {"value": "0.43239", "module": "A1-A3"}, {"value": "0.00337", "module": "A4"}, {"value": "0.028", "module": "A5"}, {"value": "0", "module": "C1"}, {"value": "0.000281", "module": "C2"}, {"value": "0.0169", "module": "C3"}, {"value": "0.00396", "module": "C4"}, {"value": "-0.0501", "module": "D", "scenario": "S0"}, {"value": "-0.00193", "module": "D", "scenario": "S1"}]}}, {"referenceToLCIAMethodDataSet": {"shortDescription": [{"value": "Auftreten von Krankheiten aufgrund von Feinstaubemissionen (PM)", "lang": "de"}, {"value": "Incidence of disease due to PM emissions (PM)", "lang": "en"}], "type": "LCIA method data set", "refObjectId": "b5c602c6-def3-11e6-bf01-fe55135034f3", "uri": "../lciamethods/b5c602c6-def3-11e6-bf01-fe55135034f3.xml"}, "other": {"anies": [{"name": "referenceToUnitGroupDataSet", "value": {"shortDescription": [{"value": "Krankheitsfälle", "lang": "de"}], "type": "unit group data set", "refObjectId": "3883559b-648f-4afc-8ba2-0bd24f3affa3", "uri": "../unitgroups/3883559b-648f-4afc-8ba2-0bd24f3affa3.xml"}}, {"module": "A1-A3"}, {"module": "A4"}, {"module": "A5"}, {"module": "C1"}, {"module": "C2"}, {"module": "C3"}, {"module": "C4"}, {"module": "D", "scenario": "S0"}, {"module": "D", "scenario": "S1"}]}}, {"referenceToLCIAMethodDataSet": {"shortDescription": [{"value": "Wirkung durch Exposition des Menschen mit U235 (IR)", "lang": "de"}, {"value": "Human exposure efficiency relative to U235 (IR)", "lang": "en"}], "type": "LCIA method data set", "refObjectId": "b5c632be-def3-11e6-bf01-fe55135034f3", "uri": "../lciamethods/b5c632be-def3-11e6-bf01-fe55135034f3.xml"}, "other": {"anies": [{"name": "referenceToUnitGroupDataSet", "value": {"shortDescription": [{"value": "kBq U235-Äq.", "lang": "de"}], "type": "unit group data set", "refObjectId": "456b05bf-1415-44a9-9993-02452f554c09", "uri": "../unitgroups/456b05bf-1415-44a9-9993-02452f554c09.xml"}}, {"module": "A1-A3"}, {"module": "A4"}, {"module": "A5"}, {"module": "C1"}, {"module": "C2"}, {"module": "C3"}, {"module": "C4"}, {"module": "D", "scenario": "S0"}, {"module": "D", "scenario": "S1"}]}}, {"referenceToLCIAMethodDataSet": {"shortDescription": [{"value": "Toxizitätsvergleichseinheit für Ökosysteme (ETP-fw)", "lang": "de"}, {"value": "Comparative toxic unit for ecosystems (ETP-fw)", "lang": "en"}], "type": "LCIA method data set", "refObjectId": "ee1082d1-b0f7-43ca-a1f0-21e2a4a74511", "uri": "../lciamethods/ee1082d1-b0f7-43ca-a1f0-21e2a4a74511.xml"}, "other": {"anies": [{"name": "referenceToUnitGroupDataSet", "value": {"shortDescription": [{"value": "CTUe", "lang": "de"}], "type": "unit group data set", "refObjectId": "aa959ded-f1eb-4efb-9c5c-2d60be36b3e6", "uri": "../unitgroups/aa959ded-f1eb-4efb-9c5c-2d60be36b3e6.xml"}}, {"module": "A1-A3"}, {"module": "A4"}, {"module": "A5"}, {"module": "C1"}, {"module": "C2"}, {"module": "C3"}, {"module": "C4"}, {"module": "D", "scenario": "S0"}, {"module": "D", "scenario": "S1"}]}}, {"referenceToLCIAMethodDataSet": {"shortDescription": [{"value": "Toxizitätsvergleichseinheit für Menschen (krebserregend) (HTP-c)", "lang": "de"}, {"value": "Comparative toxic unit for humans (carcinogenic) (HTP-c)", "lang": "en"}], "type": "LCIA method data set", "refObjectId": "2299222a-bbd8-474f-9d4f-4dd1f18aea7c", "uri": "../lciamethods/2299222a-bbd8-474f-9d4f-4dd1f18aea7c.xml"}, "other": {"anies": [{"name": "referenceToUnitGroupDataSet", "value": {"shortDescription": [{"value": "CTUh", "lang": "de"}], "type": "unit group data set", "refObjectId": "d4c9523e-2d7e-49fd-8469-998f547d3a70", "uri": "../unitgroups/d4c9523e-2d7e-49fd-8469-998f547d3a70.xml"}}, {"module": "A1-A3"}, {"module": "A4"}, {"module": "A5"}, {"module": "C1"}, {"module": "C2"}, {"module": "C3"}, {"module": "C4"}, {"module": "D", "scenario": "S0"}, {"module": "D", "scenario": "S1"}]}}, {"referenceToLCIAMethodDataSet": {"shortDescription": [{"value": "Toxizitätsvergleichseinheit für Menschen (nicht krebserregend) (HTP-nc)", "lang": "de"}, {"value": "Comparative toxic unit for humans (noncarcinogenic) (HTP-nc)", "lang": "en"}], "type": "LCIA method data set", "refObjectId": "3af763a5-b7a1-48c9-9cee-1f223481fcef", "uri": "../lciamethods/3af763a5-b7a1-48c9-9cee-1f223481fcef.xml"}, "other": {"anies": [{"name": "referenceToUnitGroupDataSet", "value": {"shortDescription": [{"value": "CTUh", "lang": "de"}], "type": "unit group data set", "refObjectId": "d4c9523e-2d7e-49fd-8469-998f547d3a70", "uri": "../unitgroups/d4c9523e-2d7e-49fd-8469-998f547d3a70.xml"}}, {"module": "A1-A3"}, {"module": "A4"}, {"module": "A5"}, {"module": "C1"}, {"module": "C2"}, {"module": "C3"}, {"module": "C4"}, {"module": "D", "scenario": "S0"}, {"module": "D", "scenario": "S1"}]}}, {"referenceToLCIAMethodDataSet": {"shortDescription": [{"value": "Bodenqualitätsindex (SQP)", "lang": "de"}, {"value": "Soil quality index (SQP)", "lang": "en"}], "type": "LCIA method data set", "refObjectId": "b2ad6890-c78d-11e6-9d9d-cec0c932ce01", "uri": "../lciamethods/b2ad6890-c78d-11e6-9d9d-cec0c932ce01.xml"}, "other": {"anies": [{"name": "referenceToUnitGroupDataSet", "value": {"shortDescription": [{"value": "SQP", "lang": "de"}], "type": "unit group data set", "refObjectId": "f130951c-e67f-4f7f-8dd4-665de3974e18", "uri": "../unitgroups/f130951c-e67f-4f7f-8dd4-665de3974e18.xml"}}, {"module": "A1-A3"}, {"module": "A4"}, {"module": "A5"}, {"module": "C1"}, {"module": "C2"}, {"module": "C3"}, {"module": "C4"}, {"module": "D", "scenario": "S0"}, {"module": "D", "scenario": "S1"}]}}]}, "otherAttributes": {"{http://www.indata.network/EPD/2019}epd-version": "1.2"}, "version": "1.1", "locations": "../ILCDLocations.xml"}