{"processInformation": {"dataSetInformation": {"UUID": "ad7a3d15-b084-43cb-a3cd-5375ddbaf315", "name": {"baseName": [{"value": "RE-PIPE", "lang": "de"}, {"value": "RE-PIPE", "lang": "en"}], "functionalUnitFlowProperties": [{"lang": "de"}]}, "classificationInformation": {"classification": [{"class": [{"value": "Kunststoffe", "level": 0, "classId": "6"}, {"value": "Rohre", "level": 1, "classId": "6.1"}, {"value": "Abwasserrohre", "level": 2, "classId": "6.1.02"}], "name": "OEKOBAU.DAT"}, {"class": [{"value": "03 Gebäudetechnik", "level": 0}, {"value": "Anlagen zur Wasserversorgung und -entsorgung", "level": 1}, {"value": "Kunststoffrohrsysteme der Warm- und Kaltwasser -installation im Gebäude ", "level": 2}], "name": "IBUCategories"}]}, "generalComment": [{"value": "Bei dem von der Studie umfassten Rohr fr Warm- und Kaltwasserinstallation im Gebude handelt es sich um ein sechsschichtiges Vollkunststoffrohr. Das Rohr kann universell fr die Heizungsinstallation eingesetzt werden. Die Handelsbezeichnung lautet \"RE-PIPE-Rohr\" Das RE-PIPE-Rohr besitzt ein Innenrohr aus Polyethylen mit erhhter Temperaturstabilitt (PE‑RT, Neuware), eine Haftvermittlerschicht, eine EVOH-Sauerstoff-Sperrschicht, eine zweite Haftvermittlerschicht, eine Schicht aus recyceltem PE-RT und eine Auenschicht aus PE-RT (Neuware).", "lang": "de"}, {"value": "The pipe covered by the study for hot and cold water installations in buildings is a six-layer solid plastic pipe. The pipe can be used universally for heating installations. The RE-PIPE pipe has an inner pipe made of polyethylene with increased temperature stability (PE-RT, virgin material), an adhesion layer, an EVOH oxygen barrier layer, a second adhesion layer, a layer of recycled PE-RT and an outer layer of PE-RT (virgin material).", "lang": "en"}], "other": {"anies": [{"scenario": [{"description": [{"value": "100 % Thermische Verwertung", "lang": "de"}, {"value": "100 % Thermal recovery", "lang": "en"}], "name": "S0", "default": true}, {"description": [{"value": "100 % Recycling", "lang": "de"}, {"value": "100 % Recycling", "lang": "en"}], "name": "S1"}, {"description": [{"value": "100 % Deponierung", "lang": "de"}, {"value": "100 % Landfill", "lang": "en"}], "name": "S2"}]}]}}, "quantitativeReference": {"referenceToReferenceFlow": [0]}, "time": {"referenceYear": 2024, "dataSetValidUntil": 2029, "other": {"anies": [{"name": "publicationDateOfEPD", "value": 1734566400000}]}}, "geography": {"locationOfOperationSupplyOrProduction": {"location": "GLO"}}, "technology": {"technologyDescriptionAndIncludedProcesses": [{"value": "Das RE-PIPE-Rohr wird in einem Produktionsschritt hergestellt. Hierfür werden PE-RT, recyceltes PE-RT, Farbmasterbatch, Haftvermittler und EVOH mittels Extrusion zu einem sechsschichtigen Rohr verarbeitet. Mit dem Farbmasterbatch wird in einem vorgelagerten Prozessschritt die Haftvermittlerschicht eingefärbt. \nTechnische Daten: \nDie in der folgenden Tabelle angegebenen Werte gelten fr das RE-PIPE-Rohr mit der Produktabmessung 16 x 2,0 mm. \nDeklarierte Einheit: \nAls deklarierte Einheit wird \"1 kg Rohr\" festgelegt. Dies entspricht 0,99 kg eingebautem Rohr (siehe Szenarioinformationen zu Modul A5 in Kapitel 4).", "lang": "de"}, {"value": "The RE-PIPE pipe is manufactured in a single production step. For this, PE-RT, recycled PE-RT, colour masterbatch, bonding agent and EVOH are processed into a five-layer pipe using extrusion. The adhesive layer is coloured with the colour masterbatch in an upstream process step. \nTechnical data: \nThe values given in the following table apply to RE-PIPE pipe with product dimensions of 16 x 2.0 mm. \nDeclared unit: \nThe declared unit is set to \"1 kg pipe\". This corresponds to 0.99 kg of installed pipe (see scenario information on module A5 in chapter 4).", "lang": "en"}], "technologicalApplicability": [{"value": "Das RE-PIPE-Rohr ist universell einsetzbar fr die Heizungsinstallation im Hochbau gem der DIN EN ISO 22391. Das Rohr ist sauerstoffdicht nach DIN 4726.", "lang": "de"}, {"value": "The RE-PIPE pipe can be used universally for heating installations in building construction in accordance with DIN EN ISO 22391. The pipe is oxygen-tight in accordance with DIN 4726.", "lang": "en"}]}}, "modellingAndValidation": {"LCIMethodAndAllocation": {"typeOfDataSet": "EPD", "referenceToLCAMethodDetails": [{"shortDescription": [{"value": "Kunststoffrohrsysteme der Warm- und Kaltwasser -installation im Gebäude .pdf", "lang": "de"}], "type": "source data set", "refObjectId": "eadd89d6-d33e-4b0c-af9c-e1b5ec2ebf9a"}], "other": {"anies": [{"name": "subType", "value": "specific dataset"}]}}, "dataSourcesTreatmentAndRepresentativeness": {"referenceToDataSource": [{"shortDescription": [{"value": "GaBi Database (all versions)", "lang": "de"}], "type": "source data set", "refObjectId": "28d74cc0-db8b-4d7e-bc44-5f6d56ce0c4a"}, {"shortDescription": [{"value": "Sphera MLC (fka GaBi) CUP 2023.02", "lang": "de"}], "type": "source data set", "refObjectId": "cb600d3b-e85a-42b3-b059-5591e2757fbb"}], "useAdviceForDataSet": [{"value": "Gültigkeitsbereich: \nDie EPD gilt fr das PE-RT-Rohr mit den Rohrgren\n\n16 x 2,0 mm\n\n20 x 2,0 mmhergestellt im Werk der Firma MAINCOR Rohrsysteme GmbH & Co. KG in Knetzgau (D). Es handelt sich um eine reprsentative EPD. \nSystemgrenze: \nBetrachtung des gesamten Produktlebenszyklus bei Nichtbetrachtung der Nutzungsphase - siehe Abbildung.\nTyp der EPD: Wiege bis Werkstor mit Optionen (Modul A4, A5, C1-C4 und D).\n\nDas nachfolgende Flieschema zeigt die Systemgrenzen bei der Bilanzierung des RE-PIPE-Rohrs.\n\n\nIm Folgenden sind die bercksichtigten Lebenswegabschnitte bzw. Prozessmodule fr die Herstellung des Rohrs detailliert aufgelistet:\n\nA1 - A3 Herstellungsphase:\nExterne Produktion der Roh-, Hilfs- und Betriebsstoffe inkl. Transport zum Werk\nExterne Regranulierung von Kunststoffmahlgut fr den Einsatz als Rezyklat\n\nExterne Produktion der Verpackungsmaterialien der Rohstoffe inkl. Transporte zur Verwertung mit anschlieender Verwertung\nRcktransport der Mehrwegverpackungen der Rohstoffe\nExterne Produktion der Verpackungsmaterialien fr das Endprodukt\nEnergiebereitstellung fr die Produktion\nProduktion der Rohre mittels Extrusion\nExterne Aufbereitung bzw. thermische Verwertung der Produktionsabflle inkl. Transport \n\nA4 und A5 Bauphase:\n\nTransport des Rohrs zur Baustelle\nTransport der Verpackung der Rohre zur Verwertung mit anschlieender Verwertung\nEnergiebereitstellung fr die Installation\nTransport und Verwertung von Montageabfllen\nSplvorgang des installierten Rohrs mit Leitungswasser\n\nC1 - C4 Entsorgung:\nEs werden drei 100%-Entsorgungsszenarien angenommen:\nEoL-Szenario 1 (Thermische Verwertung): Rckbau des Rohrs inkl. Transport zum Ort der Verwertung mit energetischer Verwertung (Modul C1, C2, C3, C4 und D).\nEoL-Szenario 2 (Recycling): Rckbau des Rohrs inkl. Transport zum Ort der Verwertung mit werkstofflicher Verwertung, d. h. Waschen, Trocknen, Schreddern und Mahlen (Modul C1, C2/1, C3/1, C4/1 und D/1).\nEoL-Szenario 3 (Deponierung): Rckbau des Rohrs inkl. Transport zum Ort der Entsorgung. Die Entsorgung findet auf einer lokalen Deponie statt (Modul C1, C2/2, C3/2, C4/2 und D/2).\n\nD Wiederverwendungs-, Rckgewinnungs- und/oder Recyclingpotentiale:\nWiederverwendungs-, Rckgewinnungs-, und/oder Recyclingpotentiale sind in den Entsorgungsszenarien vorhanden, da hier die Rohre einer energetischen bzw. stofflichen Verwertung zugefhrt werden, aus denen Energie bzw. Sekundrmaterialien zurckgewonnen werden, die auerhalb der Systemgrenze genutzt werden kann. Zurckgewonnene Energie aus der Verbrennung der Verpackungsabflle in Modul A5 werden nicht bercksichtigt. In den EoL-Szenarien 1 und 2 ergeben sich Effekte aus der Rckgewinnung von Energie bei der Verbrennung von Abfllen. Im EoL-Szenario 2 werden Vorteile aus der Nachnutzung von Sekundrmaterial bercksichtigt.", "lang": "de"}, {"value": "Scope: \nThe EPD applies to the RE-PIPE pipe with the pipe size\n\n16 x 2.0 mm\n\n20 x 2.0 mmmanufactured in the factory of MAINCOR Rohrsysteme GmbH & Co. KG in Knetzgau (Germany). This is a representative EPD. \nSystem boundary: \nConsideration of the entire product life cycle without taking the utilisation phase into account - see illustration.\nType of EPD: cradle to gate with options (modules A4, A5, C1-C4 and D).\n\nThe following flow chart shows the system boundaries when balancing the RE-PIPE pipe.\n\nThe following is a detailed list of the life cycle stages and process modules taken into account in the manufacture of the pipe:\n\nA1 - A3 Production stage:\nExternal production of raw, auxiliary and operating materials incl. transport to the plant\nExternal regranulation of plastic regrind for use as recyclate\n\nExternal production of the packaging materials of the raw materials incl. transport for recycling with subsequent recycling\nReturn transport of the reusable packaging of the raw materials\nExternal production of packaging materials for the end product\nEnergy supply for production\nProduction of the pipes by extrusion\nExternal processing or thermal utilisation of production waste incl. transport\nA4 and A5 Construction process stage:\nTransport of the pipe to the construction site\nTransport of the pipe packaging for recycling with subsequent recycling\nProvision of energy for the installation\nTransport and recycling of installation waste\nFlushing of the installed pipe with tap water\n\nC1 - C4 End of life stage:\nThree 100% End of Life scenarios are assumed:\nEoL scenario 1 (thermal utilisation): Dismantling of the pipe incl. transport to the recycling site with energy recovery (module C1, C2, C3, C4 and D).\n\nEoL scenario 2 (recycling): Dismantling of the pipe incl. transport to the recycling site with mechanical recycling, i.e. washing, drying, shredding and grinding (module C1, C2/1, C3/1, C4/1 and D/1).\nEoL scenario 3 (landfill): Dismantling of the pipe incl. transport to the disposal site. Disposal takes place at a local landfill (module C1, C2/2, C3/2, C4/2 and D/2).\n\nD Reuse, recovery and/or recycling potentials:\nReuse, recovery and/or recycling potentials are present in the EoL scenarios, as here the pipes are sent for energy or material recovery, from which energy or secondary materials are recovered that can be used outside the system boundary. Energy recovered from the incineration of packaging waste in Module A5 is not taken into account. In EoL scenarios 1 and 2, there are effects from the recovery of energy from the incineration of waste. In EoL scenario 2, benefits from the subsequent utilisation of secondary material are taken into account.", "lang": "en"}], "other": {"anies": [{"name": "referenceToOriginalEPD", "value": {"shortDescription": {"value": "RE-PIPE.pdf", "defaultValue": "RE-PIPE.pdf", "lstrings": [{"lang": "de", "value": "RE-PIPE.pdf"}]}, "type": "source data set", "uuid": {"uuid": "024ed2f8-874e-44cc-8bad-7896c1f51613"}, "refObjectId": "024ed2f8-874e-44cc-8bad-7896c1f51613", "resourceURLs": ["https://oekobaudat.de/OEKOBAU.DAT/resource/sources/024ed2f8-874e-44cc-8bad-7896c1f51613/RE-PIPE_23847.pdf?version=00.02.000"]}}]}}, "validation": {"review": [{"referenceToNameOfReviewerAndInstitution": [{"shortDescription": [{"value": "Institut Bauen und Umwelt e. V.", "lang": "de"}], "type": "contact data set", "refObjectId": "d111dbec-b024-4be5-86c5-752d6eb2cf95", "uri": "../contacts/d111dbec-b024-4be5-86c5-752d6eb2cf95.xml"}], "type": "Accredited third party review"}]}, "complianceDeclarations": {"compliance": [{"referenceToComplianceSystem": {"shortDescription": [{"value": "DIN EN 15804+A2", "lang": "de"}], "type": "source data set", "refObjectId": "c0016b33-8cf7-415c-ac6e-deba0d21440d", "uri": "../sources/c0016b33-8cf7-415c-ac6e-deba0d21440d.xml"}}, {"referenceToComplianceSystem": {"shortDescription": [{"value": "ISO 14025", "lang": "de"}], "type": "source data set", "refObjectId": "4f2eb655-6e44-4874-a95a-e28f5442cd4d", "uri": "../sources/4f2eb655-6e44-4874-a95a-e28f5442cd4d.xml"}}]}}, "administrativeInformation": {"commissionerAndGoal": {"referenceToCommissioner": [{"shortDescription": [{"value": "MAINCOR Rohrsysteme GmbH & Co. KG", "lang": "de"}], "type": "contact data set", "refObjectId": "a1819b2a-6070-47ff-bae5-d96e4c2d8168", "uri": "../contacts/a1819b2a-6070-47ff-bae5-d96e4c2d8168.xml"}]}, "dataGenerator": {"referenceToPersonOrEntityGeneratingTheDataSet": [{"shortDescription": [{"value": "SKZ - Das Kunststoff-Zentrum", "lang": "de"}], "type": "contact data set", "refObjectId": "2da43b2d-777d-45c6-ba4b-76c55a616a00", "uri": "../contacts/2da43b2d-777d-45c6-ba4b-76c55a616a00.xml"}]}, "dataEntryBy": {"timeStamp": 1734566400000, "referenceToDataSetFormat": [{"shortDescription": [{"value": "ILCD Format", "lang": "de"}], "type": "source data set", "refObjectId": "a97a0155-0234-4b87-b4ce-a45da52f2a40", "uri": "../sources/a97a0155-0234-4b87-b4ce-a45da52f2a40.xml"}, {"shortDescription": [{"value": "EPD-Datenformaterweiterungen v1.2", "lang": "de"}, {"value": "EPD Data Format Extensions v1.2", "lang": "en"}], "type": "source data set", "refObjectId": "a29449fd-aa2f-4de8-b5d7-4b06b43c6fde", "uri": "../sources/a29449fd-aa2f-4de8-b5d7-4b06b43c6fde.xml"}]}, "publicationAndOwnership": {"dataSetVersion": "00.05.000", "referenceToRegistrationAuthority": {"shortDescription": [{"value": "Institut Bauen und Umwelt e. V.", "lang": "de"}], "type": "contact data set", "refObjectId": "d111dbec-b024-4be5-86c5-752d6eb2cf95", "uri": "../contacts/d111dbec-b024-4be5-86c5-752d6eb2cf95.xml"}, "registrationNumber": "EPD-MAI-20240493-IBC2-DE", "referenceToOwnershipOfDataSet": {"shortDescription": [{"value": "MAINCOR Rohrsysteme GmbH & Co. KG", "lang": "de"}], "type": "contact data set", "refObjectId": "a1819b2a-6070-47ff-bae5-d96e4c2d8168", "uri": "../contacts/a1819b2a-6070-47ff-bae5-d96e4c2d8168.xml"}, "copyright": true, "licenseType": "Free of charge for all users and uses", "accessRestrictions": [{"value": "None", "lang": "en"}], "other": {"anies": [{"name": "referenceToPublisher", "value": {"shortDescription": [{"value": "Institut Bauen und Umwelt e. V.", "lang": "de"}], "type": "contact data set", "refObjectId": "d111dbec-b024-4be5-86c5-752d6eb2cf95", "uri": "../contacts/d111dbec-b024-4be5-86c5-752d6eb2cf95.xml"}}]}}}, "exchanges": {"exchange": [{"dataSetInternalID": 0, "referenceToFlowDataSet": {"shortDescription": [{"value": "RE-PIPE-Rohr (RE-PIPE-Rohr)", "lang": "de"}], "type": "flow data set", "refObjectId": "74540548-eeab-9300-892a-ad3f4895b27b", "uri": "../flows/74540548-eeab-9300-892a-ad3f4895b27b.xml"}, "meanAmount": 1.0, "referencesToDataSource": {}, "referenceFlow": true, "resolvedFlowVersion": "00.05.000", "resultingflowAmount": 1.0, "flowProperties": [{"name": [{"lang": "en", "value": "Mass"}, {"lang": "de", "value": "Masse"}], "uuid": "93a60a56-a3c8-11da-a746-0800200b9a66", "referenceFlowProperty": true, "meanValue": 1.0, "referenceUnit": "kg", "unitGroupUUID": "ad38d542-3fe9-439d-9b95-2f5f7752acaf"}], "materialProperties": [{"name": "gross density", "value": "946.0", "unit": "kg/m^3", "unitDescription": "kilograms per cubic metre"}], "typeOfFlow": "Product flow", "classification": {"classHierarchy": "Kunststoffe / Rohre / Abwasserrohre", "name": "OEKOBAU.DAT"}}, {"dataSetInternalID": 1, "referenceToFlowDataSet": {"shortDescription": [{"value": "Erneuerbare Primärenergie als Energieträger (PERE)", "lang": "de"}, {"value": "Renewable primary energy as energy carrier (PERE)", "lang": "en"}], "type": "flow data set", "refObjectId": "20f32be5-0398-4288-9b6d-accddd195317", "uri": "../flows/20f32be5-0398-4288-9b6d-accddd195317.xml"}, "exchange direction": "INPUT", "other": {"anies": [{"name": "referenceToUnitGroupDataSet", "value": {"shortDescription": [{"value": "MJ", "lang": "de"}], "type": "unit group data set", "refObjectId": "93a60a57-a3c8-11da-a746-0800200c9a66", "uri": "../unitgroups/93a60a57-a3c8-11da-a746-0800200c9a66.xml"}}, {"value": "5.14063721070142", "module": "A1-A3"}, {"value": "0.0950278349317407", "module": "A4"}, {"value": "0.805278792066539", "module": "A5"}, {"value": "0.0262787454558428", "module": "C1"}, {"value": "0.00772655038883409", "module": "C2", "scenario": "S0"}, {"value": "0.0218751686333225", "module": "C2", "scenario": "S1"}, {"value": "0.00772655038883409", "module": "C2", "scenario": "S2"}, {"value": "0.103795683142926", "module": "C3", "scenario": "S0"}, {"value": "0.178250213910985", "module": "C3", "scenario": "S1"}, {"value": "0", "module": "C3", "scenario": "S2"}, {"value": "0", "module": "C4", "scenario": "S0"}, {"value": "0", "module": "C4", "scenario": "S1"}, {"value": "0.0743269976575337", "module": "C4", "scenario": "S2"}, {"value": "-7.99723005728707", "module": "D", "scenario": "S0"}, {"value": "-1.25086827129521", "module": "D", "scenario": "S1"}, {"value": "0", "module": "D", "scenario": "S2"}]}, "resolvedFlowVersion": "38.00.000", "flowProperties": [], "typeOfFlow": "Other flow", "classification": {"classHierarchy": "Quantities", "name": "GaBiCategories"}}, {"dataSetInternalID": 2, "referenceToFlowDataSet": {"shortDescription": [{"value": "Erneuerbare Primärenergie zur stofflichen Nutzung (PERM)", "lang": "de"}, {"value": "Renewable primary energy resources as material utilization (PERM)", "lang": "en"}], "type": "flow data set", "refObjectId": "fb3ec0de-548d-4508-aea5-00b73bf6f702", "uri": "../flows/fb3ec0de-548d-4508-aea5-00b73bf6f702.xml"}, "exchange direction": "INPUT", "other": {"anies": [{"name": "referenceToUnitGroupDataSet", "value": {"shortDescription": [{"value": "MJ", "lang": "de"}], "type": "unit group data set", "refObjectId": "93a60a57-a3c8-11da-a746-0800200c9a66", "uri": "../unitgroups/93a60a57-a3c8-11da-a746-0800200c9a66.xml"}}, {"value": "0.727", "module": "A1-A3"}, {"value": "0", "module": "A4"}, {"value": "-0.727013821292773", "module": "A5"}, {"value": "0", "module": "C1"}, {"value": "0", "module": "C2", "scenario": "S0"}, {"value": "0", "module": "C2", "scenario": "S1"}, {"value": "0", "module": "C2", "scenario": "S2"}, {"value": "0", "module": "C3", "scenario": "S0"}, {"value": "0", "module": "C3", "scenario": "S1"}, {"value": "0", "module": "C3", "scenario": "S2"}, {"value": "0", "module": "C4", "scenario": "S0"}, {"value": "0", "module": "C4", "scenario": "S1"}, {"value": "0", "module": "C4", "scenario": "S2"}, {"value": "0", "module": "D", "scenario": "S0"}, {"value": "0", "module": "D", "scenario": "S1"}, {"value": "0", "module": "D", "scenario": "S2"}]}, "resolvedFlowVersion": "38.00.000", "flowProperties": [], "typeOfFlow": "Other flow", "classification": {"classHierarchy": "Quantities", "name": "GaBiCategories"}}, {"dataSetInternalID": 3, "referenceToFlowDataSet": {"shortDescription": [{"value": "Total erneuerbare Primärenergie (PERT)", "lang": "de"}, {"value": "Total use of renewable primary energy resources (PERT)", "lang": "en"}], "type": "flow data set", "refObjectId": "53f97275-fa8a-4cdd-9024-65936002acd0", "uri": "../flows/53f97275-fa8a-4cdd-9024-65936002acd0.xml"}, "exchange direction": "INPUT", "other": {"anies": [{"name": "referenceToUnitGroupDataSet", "value": {"shortDescription": [{"value": "MJ", "lang": "de"}], "type": "unit group data set", "refObjectId": "93a60a57-a3c8-11da-a746-0800200c9a66", "uri": "../unitgroups/93a60a57-a3c8-11da-a746-0800200c9a66.xml"}}, {"value": "5.86763721070142", "module": "A1-A3"}, {"value": "0.0950278349317407", "module": "A4"}, {"value": "0.0782649707737668", "module": "A5"}, {"value": "0.0262787454558428", "module": "C1"}, {"value": "0.00772655038883409", "module": "C2", "scenario": "S0"}, {"value": "0.0218751686333225", "module": "C2", "scenario": "S1"}, {"value": "0.00772655038883409", "module": "C2", "scenario": "S2"}, {"value": "0.103795683142926", "module": "C3", "scenario": "S0"}, {"value": "0.178250213910985", "module": "C3", "scenario": "S1"}, {"value": "0", "module": "C3", "scenario": "S2"}, {"value": "0", "module": "C4", "scenario": "S0"}, {"value": "0", "module": "C4", "scenario": "S1"}, {"value": "0.0743269976575337", "module": "C4", "scenario": "S2"}, {"value": "-7.99723005728707", "module": "D", "scenario": "S0"}, {"value": "-1.25086827129521", "module": "D", "scenario": "S1"}, {"value": "0", "module": "D", "scenario": "S2"}]}, "resolvedFlowVersion": "38.00.000", "flowProperties": [], "typeOfFlow": "Other flow", "classification": {"classHierarchy": "Quantities / Environmental quantities / EPD EN 15804 / LCI indicators", "name": "GaBiCategories"}}, {"dataSetInternalID": 4, "referenceToFlowDataSet": {"shortDescription": [{"value": "Nicht-erneuerbare Primärenergie als Energieträger (PENRE)", "lang": "de"}, {"value": "Non renewable primary energy as energy carrier (PENRE)", "lang": "en"}], "type": "flow data set", "refObjectId": "ac857178-2b45-46ec-892a-a9a4332f0372", "uri": "../flows/ac857178-2b45-46ec-892a-a9a4332f0372.xml"}, "exchange direction": "INPUT", "other": {"anies": [{"name": "referenceToUnitGroupDataSet", "value": {"shortDescription": [{"value": "MJ", "lang": "de"}], "type": "unit group data set", "refObjectId": "93a60a57-a3c8-11da-a746-0800200c9a66", "uri": "../unitgroups/93a60a57-a3c8-11da-a746-0800200c9a66.xml"}}, {"value": "55.3431785594257", "module": "A1-A3"}, {"value": "1.10331998029426", "module": "A4"}, {"value": "1.18352002319855", "module": "A5"}, {"value": "0.564523701704399", "module": "C1"}, {"value": "0.0897090566029889", "module": "C2", "scenario": "S0"}, {"value": "0.253981484927943", "module": "C2", "scenario": "S1"}, {"value": "0.0897090566029889", "module": "C2", "scenario": "S2"}, {"value": "44.167359253222", "module": "C3", "scenario": "S0"}, {"value": "5.35528092316796", "module": "C3", "scenario": "S1"}, {"value": "0", "module": "C3", "scenario": "S2"}, {"value": "0", "module": "C4", "scenario": "S0"}, {"value": "0", "module": "C4", "scenario": "S1"}, {"value": "0.491583658091543", "module": "C4", "scenario": "S2"}, {"value": "-24.0246668918791", "module": "D", "scenario": "S0"}, {"value": "-24.2884693746093", "module": "D", "scenario": "S1"}, {"value": "0", "module": "D", "scenario": "S2"}]}, "resolvedFlowVersion": "38.00.000", "flowProperties": [], "typeOfFlow": "Other flow", "classification": {"classHierarchy": "Quantities", "name": "GaBiCategories"}}, {"dataSetInternalID": 5, "referenceToFlowDataSet": {"shortDescription": [{"value": "Nicht-erneuerbare Primärenergie zur stofflichen Nutzung (PENRM)", "lang": "de"}, {"value": "Non renewable primary energy as material utilization (PENRM)", "lang": "en"}], "type": "flow data set", "refObjectId": "1421caa0-679d-4bf4-b282-0eb850ccae27", "uri": "../flows/1421caa0-679d-4bf4-b282-0eb850ccae27.xml"}, "exchange direction": "INPUT", "other": {"anies": [{"name": "referenceToUnitGroupDataSet", "value": {"shortDescription": [{"value": "MJ", "lang": "de"}], "type": "unit group data set", "refObjectId": "93a60a57-a3c8-11da-a746-0800200c9a66", "uri": "../unitgroups/93a60a57-a3c8-11da-a746-0800200c9a66.xml"}}, {"value": "33.1", "module": "A1-A3"}, {"value": "0", "module": "A4"}, {"value": "-0.482009163498097", "module": "A5"}, {"value": "0", "module": "C1"}, {"value": "0", "module": "C2", "scenario": "S0"}, {"value": "0", "module": "C2", "scenario": "S1"}, {"value": "0", "module": "C2", "scenario": "S2"}, {"value": "-32.614881254466", "module": "C3", "scenario": "S0"}, {"value": "-32.614881254466", "module": "C3", "scenario": "S1"}, {"value": "0", "module": "C3", "scenario": "S2"}, {"value": "0", "module": "C4", "scenario": "S0"}, {"value": "0", "module": "C4", "scenario": "S1"}, {"value": "0", "module": "C4", "scenario": "S2"}, {"value": "0", "module": "D", "scenario": "S0"}, {"value": "0", "module": "D", "scenario": "S1"}, {"value": "0", "module": "D", "scenario": "S2"}]}, "resolvedFlowVersion": "38.00.000", "flowProperties": [], "typeOfFlow": "Other flow", "classification": {"classHierarchy": "Quantities", "name": "GaBiCategories"}}, {"dataSetInternalID": 6, "referenceToFlowDataSet": {"shortDescription": [{"value": "Total nicht erneuerbare Primärenergie (PENRT)", "lang": "de"}, {"value": "Total use of non renewable primary energy resources (PENRT)", "lang": "en"}], "type": "flow data set", "refObjectId": "06159210-646b-4c8d-8583-da9b3b95a6c1", "uri": "../flows/06159210-646b-4c8d-8583-da9b3b95a6c1.xml"}, "exchange direction": "INPUT", "other": {"anies": [{"name": "referenceToUnitGroupDataSet", "value": {"shortDescription": [{"value": "MJ", "lang": "de"}], "type": "unit group data set", "refObjectId": "93a60a57-a3c8-11da-a746-0800200c9a66", "uri": "../unitgroups/93a60a57-a3c8-11da-a746-0800200c9a66.xml"}}, {"value": "88.4431785594254", "module": "A1-A3"}, {"value": "1.10331998029426", "module": "A4"}, {"value": "0.701510859700449", "module": "A5"}, {"value": "0.564523701704396", "module": "C1"}, {"value": "0.0897090566029889", "module": "C2", "scenario": "S0"}, {"value": "0.253981484927942", "module": "C2", "scenario": "S1"}, {"value": "0.0897090566029889", "module": "C2", "scenario": "S2"}, {"value": "11.552477998756", "module": "C3", "scenario": "S0"}, {"value": "-27.259600331298", "module": "C3", "scenario": "S1"}, {"value": "0", "module": "C3", "scenario": "S2"}, {"value": "0", "module": "C4", "scenario": "S0"}, {"value": "0", "module": "C4", "scenario": "S1"}, {"value": "0.49158365809154", "module": "C4", "scenario": "S2"}, {"value": "-24.0246668918791", "module": "D", "scenario": "S0"}, {"value": "-24.2884693746092", "module": "D", "scenario": "S1"}, {"value": "0", "module": "D", "scenario": "S2"}]}, "resolvedFlowVersion": "38.00.000", "flowProperties": [], "typeOfFlow": "Other flow", "classification": {"classHierarchy": "Quantities / Environmental quantities / EPD EN 15804 / LCI indicators", "name": "GaBiCategories"}}, {"dataSetInternalID": 7, "referenceToFlowDataSet": {"shortDescription": [{"value": "Einsatz von Sekundärstoffen (SM)", "lang": "de"}, {"value": "Use of secondary material (SM)", "lang": "en"}], "type": "flow data set", "refObjectId": "c6a1f35f-2d09-4f54-8dfb-97e502e1ce92", "uri": "../flows/c6a1f35f-2d09-4f54-8dfb-97e502e1ce92.xml"}, "exchange direction": "INPUT", "other": {"anies": [{"name": "referenceToUnitGroupDataSet", "value": {"shortDescription": [{"value": "kg", "lang": "de"}], "type": "unit group data set", "refObjectId": "ad38d542-3fe9-439d-9b95-2f5f7752acaf", "uri": "../unitgroups/ad38d542-3fe9-439d-9b95-2f5f7752acaf.xml"}}, {"value": "0.263044922667907", "module": "A1-A3"}, {"value": "0", "module": "A4"}, {"value": "0", "module": "A5"}, {"value": "0", "module": "C1"}, {"value": "0", "module": "C2", "scenario": "S0"}, {"value": "0", "module": "C2", "scenario": "S1"}, {"value": "0", "module": "C2", "scenario": "S2"}, {"value": "0", "module": "C3", "scenario": "S0"}, {"value": "0", "module": "C3", "scenario": "S1"}, {"value": "0", "module": "C3", "scenario": "S2"}, {"value": "0", "module": "C4", "scenario": "S0"}, {"value": "0", "module": "C4", "scenario": "S1"}, {"value": "0", "module": "C4", "scenario": "S2"}, {"value": "0", "module": "D", "scenario": "S0"}, {"value": "0.643599309682218", "module": "D", "scenario": "S1"}, {"value": "0", "module": "D", "scenario": "S2"}]}, "resolvedFlowVersion": "38.00.000", "flowProperties": [], "typeOfFlow": "Other flow", "classification": {"classHierarchy": "Quantities / Environmental quantities / EPD EN 15804 / LCI indicators", "name": "GaBiCategories"}}, {"dataSetInternalID": 8, "referenceToFlowDataSet": {"shortDescription": [{"value": "Erneuerbare Sekundärbrennstoffe (RSF)", "lang": "de"}, {"value": "Use of renewable secondary fuels (RSF)", "lang": "en"}], "type": "flow data set", "refObjectId": "64333088-a55f-4aa2-9a31-c10b07816787", "uri": "../flows/64333088-a55f-4aa2-9a31-c10b07816787.xml"}, "exchange direction": "INPUT", "other": {"anies": [{"name": "referenceToUnitGroupDataSet", "value": {"shortDescription": [{"value": "MJ", "lang": "de"}], "type": "unit group data set", "refObjectId": "93a60a57-a3c8-11da-a746-0800200c9a66", "uri": "../unitgroups/93a60a57-a3c8-11da-a746-0800200c9a66.xml"}}, {"value": "0", "module": "A1-A3"}, {"value": "0", "module": "A4"}, {"value": "0", "module": "A5"}, {"value": "0", "module": "C1"}, {"value": "0", "module": "C2", "scenario": "S0"}, {"value": "0", "module": "C2", "scenario": "S1"}, {"value": "0", "module": "C2", "scenario": "S2"}, {"value": "0", "module": "C3", "scenario": "S0"}, {"value": "0", "module": "C3", "scenario": "S1"}, {"value": "0", "module": "C3", "scenario": "S2"}, {"value": "0", "module": "C4", "scenario": "S0"}, {"value": "0", "module": "C4", "scenario": "S1"}, {"value": "0", "module": "C4", "scenario": "S2"}, {"value": "0", "module": "D", "scenario": "S0"}, {"value": "0", "module": "D", "scenario": "S1"}, {"value": "0", "module": "D", "scenario": "S2"}]}, "resolvedFlowVersion": "38.00.000", "flowProperties": [], "typeOfFlow": "Other flow", "classification": {"classHierarchy": "Quantities / Environmental quantities / EPD EN 15804 / LCI indicators", "name": "GaBiCategories"}}, {"dataSetInternalID": 9, "referenceToFlowDataSet": {"shortDescription": [{"value": "Nicht erneuerbare Sekundärbrennstoffe (NRSF)", "lang": "de"}, {"value": "Use of non renewable secondary fuels (NRSF)", "lang": "en"}], "type": "flow data set", "refObjectId": "89def144-d39a-4287-b86f-efde453ddcb2", "uri": "../flows/89def144-d39a-4287-b86f-efde453ddcb2.xml"}, "exchange direction": "INPUT", "other": {"anies": [{"name": "referenceToUnitGroupDataSet", "value": {"shortDescription": [{"value": "MJ", "lang": "de"}], "type": "unit group data set", "refObjectId": "93a60a57-a3c8-11da-a746-0800200c9a66", "uri": "../unitgroups/93a60a57-a3c8-11da-a746-0800200c9a66.xml"}}, {"value": "0", "module": "A1-A3"}, {"value": "0", "module": "A4"}, {"value": "0", "module": "A5"}, {"value": "0", "module": "C1"}, {"value": "0", "module": "C2", "scenario": "S0"}, {"value": "0", "module": "C2", "scenario": "S1"}, {"value": "0", "module": "C2", "scenario": "S2"}, {"value": "0", "module": "C3", "scenario": "S0"}, {"value": "0", "module": "C3", "scenario": "S1"}, {"value": "0", "module": "C3", "scenario": "S2"}, {"value": "0", "module": "C4", "scenario": "S0"}, {"value": "0", "module": "C4", "scenario": "S1"}, {"value": "0", "module": "C4", "scenario": "S2"}, {"value": "0", "module": "D", "scenario": "S0"}, {"value": "0", "module": "D", "scenario": "S1"}, {"value": "0", "module": "D", "scenario": "S2"}]}, "resolvedFlowVersion": "38.00.000", "flowProperties": [], "typeOfFlow": "Other flow", "classification": {"classHierarchy": "Quantities / Environmental quantities / EPD EN 15804 / LCI indicators", "name": "GaBiCategories"}}, {"dataSetInternalID": 10, "referenceToFlowDataSet": {"shortDescription": [{"value": "Einsatz von Süßwasserressourcen (FW)", "lang": "de"}, {"value": "Use of net fresh water (FW)", "lang": "en"}], "type": "flow data set", "refObjectId": "3cf952c8-f3a4-461d-8c96-96456ca62246", "uri": "../flows/3cf952c8-f3a4-461d-8c96-96456ca62246.xml"}, "exchange direction": "INPUT", "other": {"anies": [{"name": "referenceToUnitGroupDataSet", "value": {"shortDescription": [{"value": "m^3", "lang": "de"}], "type": "unit group data set", "refObjectId": "cd950537-0a98-4044-9ba7-9f9a68d0a504", "uri": "../unitgroups/cd950537-0a98-4044-9ba7-9f9a68d0a504.xml"}}, {"value": "0.00778402983709015", "module": "A1-A3"}, {"value": "0.000105871314933515", "module": "A4"}, {"value": "0.000480037616955739", "module": "A5"}, {"value": "7.85971549881193E-05", "module": "C1"}, {"value": "8.60821516299415E-06", "module": "C2", "scenario": "S0"}, {"value": "2.43713104614649E-05", "module": "C2", "scenario": "S1"}, {"value": "8.60821516299415E-06", "module": "C2", "scenario": "S2"}, {"value": "0.00669816908579044", "module": "C3", "scenario": "S0"}, {"value": "0.00233763801255776", "module": "C3", "scenario": "S1"}, {"value": "0", "module": "C3", "scenario": "S2"}, {"value": "0", "module": "C4", "scenario": "S0"}, {"value": "0", "module": "C4", "scenario": "S1"}, {"value": "0.000112424591241951", "module": "C4", "scenario": "S2"}, {"value": "-0.00611781286660218", "module": "D", "scenario": "S0"}, {"value": "-0.00298928495556361", "module": "D", "scenario": "S1"}, {"value": "0", "module": "D", "scenario": "S2"}]}, "resolvedFlowVersion": "38.00.000", "flowProperties": [], "typeOfFlow": "Other flow", "classification": {"classHierarchy": "Quantities / Environmental quantities / EPD EN 15804 / LCI indicators", "name": "GaBiCategories"}}, {"dataSetInternalID": 11, "referenceToFlowDataSet": {"shortDescription": [{"value": "Gefährlicher Abfall zur Deponie (HWD)", "lang": "de"}, {"value": "Hazardous waste disposed (HWD)", "lang": "en"}], "type": "flow data set", "refObjectId": "430f9e0f-59b2-46a0-8e0d-55e0e84948fc", "uri": "../flows/430f9e0f-59b2-46a0-8e0d-55e0e84948fc.xml"}, "exchange direction": "OUTPUT", "other": {"anies": [{"name": "referenceToUnitGroupDataSet", "value": {"shortDescription": [{"value": "kg", "lang": "de"}], "type": "unit group data set", "refObjectId": "ad38d542-3fe9-439d-9b95-2f5f7752acaf", "uri": "../unitgroups/ad38d542-3fe9-439d-9b95-2f5f7752acaf.xml"}}, {"value": "7.29394230537924E-09", "module": "A1-A3"}, {"value": "4.22454378986709E-11", "module": "A4"}, {"value": "1.71558951866267E-10", "module": "A5"}, {"value": "6.43205392927831E-11", "module": "C1"}, {"value": "3.43490415052501E-12", "module": "C2", "scenario": "S0"}, {"value": "9.72479356901886E-12", "module": "C2", "scenario": "S1"}, {"value": "3.43490415052501E-12", "module": "C2", "scenario": "S2"}, {"value": "2.15670757401772E-10", "module": "C3", "scenario": "S0"}, {"value": "4.3325378516994E-10", "module": "C3", "scenario": "S1"}, {"value": "0", "module": "C3", "scenario": "S2"}, {"value": "0", "module": "C4", "scenario": "S0"}, {"value": "0", "module": "C4", "scenario": "S1"}, {"value": "1.21509322891669E-10", "module": "C4", "scenario": "S2"}, {"value": "-1.61502758648286E-08", "module": "D", "scenario": "S0"}, {"value": "-2.93907137705248E-09", "module": "D", "scenario": "S1"}, {"value": "0", "module": "D", "scenario": "S2"}]}, "resolvedFlowVersion": "38.00.000", "flowProperties": [], "typeOfFlow": "Other flow", "classification": {"classHierarchy": "Quantities / Environmental quantities / EPD EN 15804 / LCI indicators", "name": "GaBiCategories"}}, {"dataSetInternalID": 12, "referenceToFlowDataSet": {"shortDescription": [{"value": "Entsorgter nicht gefährlicher Abfall (NHWD)", "lang": "de"}, {"value": "Non hazardous waste disposed (NHWD)", "lang": "en"}], "type": "flow data set", "refObjectId": "b29ef66b-e286-4afa-949f-62f1a7b4d7fa", "uri": "../flows/b29ef66b-e286-4afa-949f-62f1a7b4d7fa.xml"}, "exchange direction": "OUTPUT", "other": {"anies": [{"name": "referenceToUnitGroupDataSet", "value": {"shortDescription": [{"value": "kg", "lang": "de"}], "type": "unit group data set", "refObjectId": "ad38d542-3fe9-439d-9b95-2f5f7752acaf", "uri": "../unitgroups/ad38d542-3fe9-439d-9b95-2f5f7752acaf.xml"}}, {"value": "0.0146121260418809", "module": "A1-A3"}, {"value": "0.000180157856543029", "module": "A4"}, {"value": "0.0185384288230534", "module": "A5"}, {"value": "0.000154635018733984", "module": "C1"}, {"value": "1.46483265405756E-05", "module": "C2", "scenario": "S0"}, {"value": "4.14718855304608E-05", "module": "C2", "scenario": "S1"}, {"value": "1.46483265405756E-05", "module": "C2", "scenario": "S2"}, {"value": "0.0122941830875903", "module": "C3", "scenario": "S0"}, {"value": "0.00205175359494159", "module": "C3", "scenario": "S1"}, {"value": "0", "module": "C3", "scenario": "S2"}, {"value": "0", "module": "C4", "scenario": "S0"}, {"value": "0", "module": "C4", "scenario": "S1"}, {"value": "0.985919903204322", "module": "C4", "scenario": "S2"}, {"value": "-0.0124958737614959", "module": "D", "scenario": "S0"}, {"value": "-0.00498395481934696", "module": "D", "scenario": "S1"}, {"value": "0", "module": "D", "scenario": "S2"}]}, "resolvedFlowVersion": "38.00.000", "flowProperties": [], "typeOfFlow": "Other flow", "classification": {"classHierarchy": "Quantities / Environmental quantities / EPD EN 15804 / LCI indicators", "name": "GaBiCategories"}}, {"dataSetInternalID": 13, "referenceToFlowDataSet": {"shortDescription": [{"value": "Entsorgter radioaktiver Abfall (RWD)", "lang": "de"}, {"value": "Radioactive waste disposed (RWD)", "lang": "en"}], "type": "flow data set", "refObjectId": "3449546e-52ad-4b39-b809-9fb77cea8ff6", "uri": "../flows/3449546e-52ad-4b39-b809-9fb77cea8ff6.xml"}, "exchange direction": "OUTPUT", "other": {"anies": [{"name": "referenceToUnitGroupDataSet", "value": {"shortDescription": [{"value": "kg", "lang": "de"}], "type": "unit group data set", "refObjectId": "ad38d542-3fe9-439d-9b95-2f5f7752acaf", "uri": "../unitgroups/ad38d542-3fe9-439d-9b95-2f5f7752acaf.xml"}}, {"value": "0.000223416123480094", "module": "A1-A3"}, {"value": "2.00966495707181E-06", "module": "A4"}, {"value": "5.55453031831013E-05", "module": "A5"}, {"value": "4.58758238873234E-05", "module": "C1"}, {"value": "1.63402413268104E-07", "module": "C2", "scenario": "S0"}, {"value": "4.62619819382424E-07", "module": "C2", "scenario": "S1"}, {"value": "1.63402413268104E-07", "module": "C2", "scenario": "S2"}, {"value": "2.05723110522827E-05", "module": "C3", "scenario": "S0"}, {"value": "0.000301696035940346", "module": "C3", "scenario": "S1"}, {"value": "0", "module": "C3", "scenario": "S2"}, {"value": "0", "module": "C4", "scenario": "S0"}, {"value": "0", "module": "C4", "scenario": "S1"}, {"value": "6.93706425368593E-06", "module": "C4", "scenario": "S2"}, {"value": "-0.00176234952480603", "module": "D", "scenario": "S0"}, {"value": "-0.000234108315101408", "module": "D", "scenario": "S1"}, {"value": "0", "module": "D", "scenario": "S2"}]}, "resolvedFlowVersion": "38.00.000", "flowProperties": [], "typeOfFlow": "Other flow", "classification": {"classHierarchy": "Quantities / Environmental quantities / EPD EN 15804 / LCI indicators", "name": "GaBiCategories"}}, {"dataSetInternalID": 14, "referenceToFlowDataSet": {"shortDescription": [{"value": "Komponenten für die Wiederverwendung (CRU)", "lang": "de"}, {"value": "Components for re-use (CRU)", "lang": "en"}], "type": "flow data set", "refObjectId": "a2b32f97-3fc7-4af2-b209-525bc6426f33", "uri": "../flows/a2b32f97-3fc7-4af2-b209-525bc6426f33.xml"}, "exchange direction": "OUTPUT", "other": {"anies": [{"name": "referenceToUnitGroupDataSet", "value": {"shortDescription": [{"value": "kg", "lang": "de"}], "type": "unit group data set", "refObjectId": "ad38d542-3fe9-439d-9b95-2f5f7752acaf", "uri": "../unitgroups/ad38d542-3fe9-439d-9b95-2f5f7752acaf.xml"}}, {"value": "0", "module": "A1-A3"}, {"value": "0", "module": "A4"}, {"value": "0", "module": "A5"}, {"value": "0", "module": "C1"}, {"value": "0", "module": "C2", "scenario": "S0"}, {"value": "0", "module": "C2", "scenario": "S1"}, {"value": "0", "module": "C2", "scenario": "S2"}, {"value": "0", "module": "C3", "scenario": "S0"}, {"value": "0", "module": "C3", "scenario": "S1"}, {"value": "0", "module": "C3", "scenario": "S2"}, {"value": "0", "module": "C4", "scenario": "S0"}, {"value": "0", "module": "C4", "scenario": "S1"}, {"value": "0", "module": "C4", "scenario": "S2"}, {"value": "0", "module": "D", "scenario": "S0"}, {"value": "0", "module": "D", "scenario": "S1"}, {"value": "0", "module": "D", "scenario": "S2"}]}, "resolvedFlowVersion": "38.00.000", "flowProperties": [], "typeOfFlow": "Other flow", "classification": {"classHierarchy": "Quantities / Environmental quantities / EPD EN 15804 / LCI indicators", "name": "GaBiCategories"}}, {"dataSetInternalID": 15, "referenceToFlowDataSet": {"shortDescription": [{"value": "Stoffe zum Recycling (MFR)", "lang": "de"}, {"value": "Materials for recycling (MFR)", "lang": "en"}], "type": "flow data set", "refObjectId": "d7fe48a5-4103-49c8-9aae-b0b5dfdbd6ae", "uri": "../flows/d7fe48a5-4103-49c8-9aae-b0b5dfdbd6ae.xml"}, "exchange direction": "OUTPUT", "other": {"anies": [{"name": "referenceToUnitGroupDataSet", "value": {"shortDescription": [{"value": "kg", "lang": "de"}], "type": "unit group data set", "refObjectId": "ad38d542-3fe9-439d-9b95-2f5f7752acaf", "uri": "../unitgroups/ad38d542-3fe9-439d-9b95-2f5f7752acaf.xml"}}, {"value": "0.043028271", "module": "A1-A3"}, {"value": "0", "module": "A4"}, {"value": "0", "module": "A5"}, {"value": "0", "module": "C1"}, {"value": "0", "module": "C2", "scenario": "S0"}, {"value": "0", "module": "C2", "scenario": "S1"}, {"value": "0", "module": "C2", "scenario": "S2"}, {"value": "0", "module": "C3", "scenario": "S0"}, {"value": "0.940517880228137", "module": "C3", "scenario": "S1"}, {"value": "0", "module": "C3", "scenario": "S2"}, {"value": "0", "module": "C4", "scenario": "S0"}, {"value": "0", "module": "C4", "scenario": "S1"}, {"value": "0", "module": "C4", "scenario": "S2"}, {"value": "0", "module": "D", "scenario": "S0"}, {"value": "0", "module": "D", "scenario": "S1"}, {"value": "0", "module": "D", "scenario": "S2"}]}, "resolvedFlowVersion": "38.00.000", "flowProperties": [], "typeOfFlow": "Other flow", "classification": {"classHierarchy": "Quantities / Environmental quantities / EPD EN 15804 / LCI indicators", "name": "GaBiCategories"}}, {"dataSetInternalID": 16, "referenceToFlowDataSet": {"shortDescription": [{"value": "Stoffe für die Energierückgewinnung (MER)", "lang": "de"}, {"value": "Materials for energy recovery (MER)", "lang": "en"}], "type": "flow data set", "refObjectId": "59a9181c-3aaf-46ee-8b13-2b3723b6e447", "uri": "../flows/59a9181c-3aaf-46ee-8b13-2b3723b6e447.xml"}, "exchange direction": "OUTPUT", "other": {"anies": [{"name": "referenceToUnitGroupDataSet", "value": {"shortDescription": [{"value": "kg", "lang": "de"}], "type": "unit group data set", "refObjectId": "ad38d542-3fe9-439d-9b95-2f5f7752acaf", "uri": "../unitgroups/ad38d542-3fe9-439d-9b95-2f5f7752acaf.xml"}}, {"value": "0", "module": "A1-A3"}, {"value": "0", "module": "A4"}, {"value": "0", "module": "A5"}, {"value": "0", "module": "C1"}, {"value": "0", "module": "C2", "scenario": "S0"}, {"value": "0", "module": "C2", "scenario": "S1"}, {"value": "0", "module": "C2", "scenario": "S2"}, {"value": "0", "module": "C3", "scenario": "S0"}, {"value": "0", "module": "C3", "scenario": "S1"}, {"value": "0", "module": "C3", "scenario": "S2"}, {"value": "0", "module": "C4", "scenario": "S0"}, {"value": "0", "module": "C4", "scenario": "S1"}, {"value": "0", "module": "C4", "scenario": "S2"}, {"value": "0", "module": "D", "scenario": "S0"}, {"value": "0", "module": "D", "scenario": "S1"}, {"value": "0", "module": "D", "scenario": "S2"}]}, "resolvedFlowVersion": "38.00.000", "flowProperties": [], "typeOfFlow": "Other flow", "classification": {"classHierarchy": "Quantities / Environmental quantities / EPD EN 15804 / LCI indicators", "name": "GaBiCategories"}}, {"dataSetInternalID": 17, "referenceToFlowDataSet": {"shortDescription": [{"value": "Exportierte elektrische Energie (EEE)", "lang": "de"}, {"value": "Exported electrical energy (EEE)", "lang": "en"}], "type": "flow data set", "refObjectId": "4da0c987-2b76-40d6-9e9e-82a017aaaf29", "uri": "../flows/4da0c987-2b76-40d6-9e9e-82a017aaaf29.xml"}, "exchange direction": "OUTPUT", "other": {"anies": [{"name": "referenceToUnitGroupDataSet", "value": {"shortDescription": [{"value": "MJ", "lang": "de"}], "type": "unit group data set", "refObjectId": "93a60a57-a3c8-11da-a746-0800200c9a66", "uri": "../unitgroups/93a60a57-a3c8-11da-a746-0800200c9a66.xml"}}, {"value": "0.0760447195906894", "module": "A1-A3"}, {"value": "0", "module": "A4"}, {"value": "0.189876336572491", "module": "A5"}, {"value": "0", "module": "C1"}, {"value": "0", "module": "C2", "scenario": "S0"}, {"value": "0", "module": "C2", "scenario": "S1"}, {"value": "0", "module": "C2", "scenario": "S2"}, {"value": "6.61445434614057", "module": "C3", "scenario": "S0"}, {"value": "0.330722717307028", "module": "C3", "scenario": "S1"}, {"value": "0", "module": "C3", "scenario": "S2"}, {"value": "0", "module": "C4", "scenario": "S0"}, {"value": "0", "module": "C4", "scenario": "S1"}, {"value": "0", "module": "C4", "scenario": "S2"}, {"value": "0", "module": "D", "scenario": "S0"}, {"value": "0", "module": "D", "scenario": "S1"}, {"value": "0", "module": "D", "scenario": "S2"}]}, "resolvedFlowVersion": "38.00.000", "flowProperties": [], "typeOfFlow": "Other flow", "classification": {"classHierarchy": "Quantities / Environmental quantities / EPD EN 15804 / LCI indicators", "name": "GaBiCategories"}}, {"dataSetInternalID": 18, "referenceToFlowDataSet": {"shortDescription": [{"value": "Exportierte thermische Energie (EET)", "lang": "de"}, {"value": "Exported thermal energy (EET)", "lang": "en"}], "type": "flow data set", "refObjectId": "98daf38a-7a79-46d3-9a37-2b7bd0955810", "uri": "../flows/98daf38a-7a79-46d3-9a37-2b7bd0955810.xml"}, "exchange direction": "OUTPUT", "other": {"anies": [{"name": "referenceToUnitGroupDataSet", "value": {"shortDescription": [{"value": "MJ", "lang": "de"}], "type": "unit group data set", "refObjectId": "93a60a57-a3c8-11da-a746-0800200c9a66", "uri": "../unitgroups/93a60a57-a3c8-11da-a746-0800200c9a66.xml"}}, {"value": "0.175142369192818", "module": "A1-A3"}, {"value": "0", "module": "A4"}, {"value": "0.376887068330411", "module": "A5"}, {"value": "0", "module": "C1"}, {"value": "0", "module": "C2", "scenario": "S0"}, {"value": "0", "module": "C2", "scenario": "S1"}, {"value": "0", "module": "C2", "scenario": "S2"}, {"value": "11.7614085709972", "module": "C3", "scenario": "S0"}, {"value": "0.588070428549861", "module": "C3", "scenario": "S1"}, {"value": "0", "module": "C3", "scenario": "S2"}, {"value": "0", "module": "C4", "scenario": "S0"}, {"value": "0", "module": "C4", "scenario": "S1"}, {"value": "0", "module": "C4", "scenario": "S2"}, {"value": "0", "module": "D", "scenario": "S0"}, {"value": "0", "module": "D", "scenario": "S1"}, {"value": "0", "module": "D", "scenario": "S2"}]}, "resolvedFlowVersion": "38.00.000", "flowProperties": [], "typeOfFlow": "Other flow", "classification": {"classHierarchy": "Quantities / Environmental quantities / EPD EN 15804 / LCI indicators", "name": "GaBiCategories"}}]}, "LCIAResults": {"LCIAResult": [{"referenceToLCIAMethodDataSet": {"shortDescription": [{"value": "Globales Erwärmungspotenzial total (GWP-total)", "lang": "de"}, {"value": "Global Warming Potential total (GWP-total)", "lang": "en"}], "type": "LCIA method data set", "refObjectId": "6a37f984-a4b3-458a-a20a-64418c145fa2", "uri": "../lciamethods/6a37f984-a4b3-458a-a20a-64418c145fa2.xml"}, "other": {"anies": [{"name": "referenceToUnitGroupDataSet", "value": {"shortDescription": [{"value": "kg CO_(2)-Äq.", "lang": "de"}], "type": "unit group data set", "refObjectId": "1ebf3012-d0db-4de2-aefd-ef30cedb0be1", "uri": "../unitgroups/1ebf3012-d0db-4de2-aefd-ef30cedb0be1.xml"}}, {"value": "1.49541564885101", "module": "A1-A3"}, {"value": "0.0859994817092134", "module": "A4"}, {"value": "0.179582315461235", "module": "A5"}, {"value": "0.0404115429295553", "module": "C1"}, {"value": "0.00710910257754387", "module": "C2", "scenario": "S0"}, {"value": "0.0201270696351242", "module": "C2", "scenario": "S1"}, {"value": "0.00710910257754387", "module": "C2", "scenario": "S2"}, {"value": "3.0989096286157", "module": "C3", "scenario": "S0"}, {"value": "0.420324589256704", "module": "C3", "scenario": "S1"}, {"value": "0", "module": "C3", "scenario": "S2"}, {"value": "0", "module": "C4", "scenario": "S0"}, {"value": "0", "module": "C4", "scenario": "S1"}, {"value": "0.0292052691453876", "module": "C4", "scenario": "S2"}, {"value": "-1.35365942948209", "module": "D", "scenario": "S0"}, {"value": "-0.587907234897682", "module": "D", "scenario": "S1"}, {"value": "0", "module": "D", "scenario": "S2"}]}}, {"referenceToLCIAMethodDataSet": {"shortDescription": [{"value": "Globales Erwärmungspotenzial fossil (GWP-fossil)", "lang": "de"}, {"value": "Global Warming Potential fossil fuels (GWP-fossil)", "lang": "en"}], "type": "LCIA method data set", "refObjectId": "5f635281-343e-44fb-83df-1971b155e6b6", "uri": "../lciamethods/5f635281-343e-44fb-83df-1971b155e6b6.xml"}, "other": {"anies": [{"name": "referenceToUnitGroupDataSet", "value": {"shortDescription": [{"value": "kg CO_(2)-Äq.", "lang": "de"}], "type": "unit group data set", "refObjectId": "1ebf3012-d0db-4de2-aefd-ef30cedb0be1", "uri": "../unitgroups/1ebf3012-d0db-4de2-aefd-ef30cedb0be1.xml"}}, {"value": "1.56399990677479", "module": "A1-A3"}, {"value": "0.0845919829899217", "module": "A4"}, {"value": "0.109816124350683", "module": "A5"}, {"value": "0.0403975988709535", "module": "C1"}, {"value": "0.00699466126900897", "module": "C2", "scenario": "S0"}, {"value": "0.019803066969402", "module": "C2", "scenario": "S1"}, {"value": "0.00699466126900897", "module": "C2", "scenario": "S2"}, {"value": "3.0988251998069", "module": "C3", "scenario": "S0"}, {"value": "0.420218741735041", "module": "C3", "scenario": "S1"}, {"value": "0", "module": "C3", "scenario": "S2"}, {"value": "0", "module": "C4", "scenario": "S0"}, {"value": "0", "module": "C4", "scenario": "S1"}, {"value": "0.0290980732146598", "module": "C4", "scenario": "S2"}, {"value": "-1.34771782199175", "module": "D", "scenario": "S0"}, {"value": "-0.585202607774527", "module": "D", "scenario": "S1"}, {"value": "0", "module": "D", "scenario": "S2"}]}}, {"referenceToLCIAMethodDataSet": {"shortDescription": [{"value": "Globales Erwärmungspotenzial biogen (GWP-biogenic)", "lang": "de"}, {"value": "Global Warming Potential biogenic (GWP-biogenic)", "lang": "en"}], "type": "LCIA method data set", "refObjectId": "2356e1ab-0185-4db5-86e5-16de51c7485c", "uri": "../lciamethods/2356e1ab-0185-4db5-86e5-16de51c7485c.xml"}, "other": {"anies": [{"name": "referenceToUnitGroupDataSet", "value": {"shortDescription": [{"value": "kg CO_(2)-Äq.", "lang": "de"}], "type": "unit group data set", "refObjectId": "1ebf3012-d0db-4de2-aefd-ef30cedb0be1", "uri": "../unitgroups/1ebf3012-d0db-4de2-aefd-ef30cedb0be1.xml"}}, {"value": "-0.0697464105552391", "module": "A1-A3"}, {"value": "0", "module": "A4"}, {"value": "0.0697464105552391", "module": "A5"}, {"value": "9.79972133985797E-06", "module": "C1"}, {"value": "0", "module": "C2", "scenario": "S0"}, {"value": "0", "module": "C2", "scenario": "S1"}, {"value": "0", "module": "C2", "scenario": "S2"}, {"value": "7.82247552737511E-05", "module": "C3", "scenario": "S0"}, {"value": "7.08544907840275E-05", "module": "C3", "scenario": "S1"}, {"value": "0", "module": "C3", "scenario": "S2"}, {"value": "0", "module": "C4", "scenario": "S0"}, {"value": "0", "module": "C4", "scenario": "S1"}, {"value": "0", "module": "C4", "scenario": "S2"}, {"value": "-0.00581929603760536", "module": "D", "scenario": "S0"}, {"value": "-0.00263128322679695", "module": "D", "scenario": "S1"}, {"value": "0", "module": "D", "scenario": "S2"}]}}, {"referenceToLCIAMethodDataSet": {"shortDescription": [{"value": "Globales Erwärmungspotenzial luluc (GWP-luluc)", "lang": "de"}, {"value": "Global Warming Potential luluc (GWP-luluc)", "lang": "en"}], "type": "LCIA method data set", "refObjectId": "4331bbdb-978a-490d-8707-eeb047f01a55", "uri": "../lciamethods/4331bbdb-978a-490d-8707-eeb047f01a55.xml"}, "other": {"anies": [{"name": "referenceToUnitGroupDataSet", "value": {"shortDescription": [{"value": "kg CO_(2)-Äq.", "lang": "de"}], "type": "unit group data set", "refObjectId": "1ebf3012-d0db-4de2-aefd-ef30cedb0be1", "uri": "../unitgroups/1ebf3012-d0db-4de2-aefd-ef30cedb0be1.xml"}}, {"value": "0.00116215263146109", "module": "A1-A3"}, {"value": "0.00140749871929171", "module": "A4"}, {"value": "1.97805553127615E-05", "module": "A5"}, {"value": "4.14433726197329E-06", "module": "C1"}, {"value": "0.0001144413085349", "module": "C2", "scenario": "S0"}, {"value": "0.000324002665722184", "module": "C2", "scenario": "S1"}, {"value": "0.0001144413085349", "module": "C2", "scenario": "S2"}, {"value": "6.20405352204778E-06", "module": "C3", "scenario": "S0"}, {"value": "3.49930308785292E-05", "module": "C3", "scenario": "S1"}, {"value": "0", "module": "C3", "scenario": "S2"}, {"value": "0", "module": "C4", "scenario": "S0"}, {"value": "0", "module": "C4", "scenario": "S1"}, {"value": "0.000107195930727829", "module": "C4", "scenario": "S2"}, {"value": "-0.000122311452735762", "module": "D", "scenario": "S0"}, {"value": "-7.3343896357651E-05", "module": "D", "scenario": "S1"}, {"value": "0", "module": "D", "scenario": "S2"}]}}, {"referenceToLCIAMethodDataSet": {"shortDescription": [{"value": "Abbau Potential der stratosphärischen Ozonschicht (ODP)", "lang": "de"}, {"value": "Depletion potential of the stratospheric ozone layer (ODP)", "lang": "en"}], "type": "LCIA method data set", "refObjectId": "b5c629d6-def3-11e6-bf01-fe55135034f3", "uri": "../lciamethods/b5c629d6-def3-11e6-bf01-fe55135034f3.xml"}, "other": {"anies": [{"name": "referenceToUnitGroupDataSet", "value": {"shortDescription": [{"value": "kg CFC11-Äq.", "lang": "de"}], "type": "unit group data set", "refObjectId": "d9e957c9-7309-4474-bf3a-7777df6c4e5b", "uri": "../unitgroups/d9e957c9-7309-4474-bf3a-7777df6c4e5b.xml"}}, {"value": "4.47649629601574E-12", "module": "A1-A3"}, {"value": "1.233784353683E-14", "module": "A4"}, {"value": "8.66094339489369E-14", "module": "A5"}, {"value": "2.29158096880146E-15", "module": "C1"}, {"value": "1.00316891198609E-15", "module": "C2", "scenario": "S0"}, {"value": "2.84014055601257E-15", "module": "C2", "scenario": "S1"}, {"value": "1.00316891198609E-15", "module": "C2", "scenario": "S2"}, {"value": "1.64496846323347E-13", "module": "C3", "scenario": "S0"}, {"value": "2.39453906927635E-14", "module": "C3", "scenario": "S1"}, {"value": "0", "module": "C3", "scenario": "S2"}, {"value": "0", "module": "C4", "scenario": "S0"}, {"value": "0", "module": "C4", "scenario": "S1"}, {"value": "9.59995784241479E-14", "module": "C4", "scenario": "S2"}, {"value": "-1.19659432673831E-11", "module": "D", "scenario": "S0"}, {"value": "-1.89611302870399E-12", "module": "D", "scenario": "S1"}, {"value": "0", "module": "D", "scenario": "S2"}]}}, {"referenceToLCIAMethodDataSet": {"shortDescription": [{"value": "Versauerungspotenzial von Boden und Wasser (AP)", "lang": "de"}, {"value": "Acidification potential of land and water (AP)", "lang": "en"}], "type": "LCIA method data set", "refObjectId": "b5c611c6-def3-11e6-bf01-fe55135034f3", "uri": "../lciamethods/b5c611c6-def3-11e6-bf01-fe55135034f3.xml"}, "other": {"anies": [{"name": "referenceToUnitGroupDataSet", "value": {"shortDescription": [{"value": "mol H^(+)-Äq.", "lang": "de"}], "type": "unit group data set", "refObjectId": "42e089ac-92bf-4bf2-8ca1-5fc40d18f2ed", "uri": "../unitgroups/42e089ac-92bf-4bf2-8ca1-5fc40d18f2ed.xml"}}, {"value": "0.00206532897370041", "module": "A1-A3"}, {"value": "0.000185678073930864", "module": "A4"}, {"value": "0.000122626922469556", "module": "A5"}, {"value": "5.42253824215725E-05", "module": "C1"}, {"value": "1.06888450017847E-05", "module": "C2", "scenario": "S0"}, {"value": "3.02619248102477E-05", "module": "C2", "scenario": "S1"}, {"value": "1.06888450017847E-05", "module": "C2", "scenario": "S2"}, {"value": "0.000308842377613073", "module": "C3", "scenario": "S0"}, {"value": "0.000371651408701101", "module": "C3", "scenario": "S1"}, {"value": "0", "module": "C3", "scenario": "S2"}, {"value": "0", "module": "C4", "scenario": "S0"}, {"value": "0", "module": "C4", "scenario": "S1"}, {"value": "0.00017419291450889", "module": "C4", "scenario": "S2"}, {"value": "-0.0014088153697359", "module": "D", "scenario": "S0"}, {"value": "-0.00135435284741084", "module": "D", "scenario": "S1"}, {"value": "0", "module": "D", "scenario": "S2"}]}}, {"referenceToLCIAMethodDataSet": {"shortDescription": [{"value": "Eutrophierungspotenzial Süßwasser (EP-freshwater)", "lang": "de"}, {"value": "Eutrophication potential aquatic freshwater (EP-freshwater)", "lang": "en"}], "type": "LCIA method data set", "refObjectId": "b53ec18f-7377-4ad3-86eb-cc3f4f276b2b", "uri": "../lciamethods/b53ec18f-7377-4ad3-86eb-cc3f4f276b2b.xml"}, "other": {"anies": [{"name": "referenceToUnitGroupDataSet", "value": {"shortDescription": [{"value": "kg P-Äq.", "lang": "de"}], "type": "unit group data set", "refObjectId": "0429039d-a61d-4590-ba67-aa4a20a810a1", "uri": "../unitgroups/0429039d-a61d-4590-ba67-aa4a20a810a1.xml"}}, {"value": "2.43511547271437E-06", "module": "A1-A3"}, {"value": "3.57634038484662E-07", "module": "A4"}, {"value": "1.1362493708349E-05", "module": "A5"}, {"value": "1.0709775158927E-08", "module": "C1"}, {"value": "2.90786107154694E-08", "module": "C2", "scenario": "S0"}, {"value": "8.23264563113289E-08", "module": "C2", "scenario": "S1"}, {"value": "2.90786107154694E-08", "module": "C2", "scenario": "S2"}, {"value": "3.5392199580323E-08", "module": "C3", "scenario": "S0"}, {"value": "9.09306880539387E-08", "module": "C3", "scenario": "S1"}, {"value": "0", "module": "C3", "scenario": "S2"}, {"value": "0", "module": "C4", "scenario": "S0"}, {"value": "0", "module": "C4", "scenario": "S1"}, {"value": "1.66959621805433E-05", "module": "C4", "scenario": "S2"}, {"value": "-2.2422364534293E-06", "module": "D", "scenario": "S0"}, {"value": "-8.59141289662979E-07", "module": "D", "scenario": "S1"}, {"value": "0", "module": "D", "scenario": "S2"}]}}, {"referenceToLCIAMethodDataSet": {"shortDescription": [{"value": "Eutrophierungspotenzial Salzwasser (EP-marine)", "lang": "de"}, {"value": "Eutrophication potential aquatic marine (EP-marine)", "lang": "en"}], "type": "LCIA method data set", "refObjectId": "b5c619fa-def3-11e6-bf01-fe55135034f3", "uri": "../lciamethods/b5c619fa-def3-11e6-bf01-fe55135034f3.xml"}, "other": {"anies": [{"name": "referenceToUnitGroupDataSet", "value": {"shortDescription": [{"value": "kg N-Äq.", "lang": "de"}], "type": "unit group data set", "refObjectId": "d05bb823-ecdf-4686-8c40-bf1d9257859f", "uri": "../unitgroups/d05bb823-ecdf-4686-8c40-bf1d9257859f.xml"}}, {"value": "0.000591995228999769", "module": "A1-A3"}, {"value": "7.89725099336858E-05", "module": "A4"}, {"value": "8.29791774496338E-05", "module": "A5"}, {"value": "1.47335208256629E-05", "module": "C1"}, {"value": "4.09657223035281E-06", "module": "C2", "scenario": "S0"}, {"value": "1.15980876132067E-05", "module": "C2", "scenario": "S1"}, {"value": "4.09657223035281E-06", "module": "C2", "scenario": "S2"}, {"value": "6.64235882076951E-05", "module": "C3", "scenario": "S0"}, {"value": "0.000100251341857361", "module": "C3", "scenario": "S1"}, {"value": "0", "module": "C3", "scenario": "S2"}, {"value": "0", "module": "C4", "scenario": "S0"}, {"value": "0", "module": "C4", "scenario": "S1"}, {"value": "3.74855254775098E-05", "module": "C4", "scenario": "S2"}, {"value": "-0.000430845145093629", "module": "D", "scenario": "S0"}, {"value": "-0.000436197409527738", "module": "D", "scenario": "S1"}, {"value": "0", "module": "D", "scenario": "S2"}]}}, {"referenceToLCIAMethodDataSet": {"shortDescription": [{"value": "Eutrophierungspotenzial Land (EP-terrestrial)", "lang": "de"}, {"value": "Eutrophication potential terrestrial (EP-terrestrial)", "lang": "en"}], "type": "LCIA method data set", "refObjectId": "b5c614d2-def3-11e6-bf01-fe55135034f3", "uri": "../lciamethods/b5c614d2-def3-11e6-bf01-fe55135034f3.xml"}, "other": {"anies": [{"name": "referenceToUnitGroupDataSet", "value": {"shortDescription": [{"value": "mol N-Äq.", "lang": "de"}], "type": "unit group data set", "refObjectId": "71b4d617-0ec9-4d3f-b65e-e438940c2401", "uri": "../unitgroups/71b4d617-0ec9-4d3f-b65e-e438940c2401.xml"}}, {"value": "0.0062575409452416", "module": "A1-A3"}, {"value": "0.000903930052161017", "module": "A4"}, {"value": "0.000473694909084918", "module": "A5"}, {"value": "0.000159699252079061", "module": "C1"}, {"value": "4.80954106241858E-05", "module": "C2", "scenario": "S0"}, {"value": "0.000136166227481461", "module": "C2", "scenario": "S1"}, {"value": "4.80954106241858E-05", "module": "C2", "scenario": "S2"}, {"value": "0.00146657557911225", "module": "C3", "scenario": "S0"}, {"value": "0.00112352513901836", "module": "C3", "scenario": "S1"}, {"value": "0", "module": "C3", "scenario": "S2"}, {"value": "0", "module": "C4", "scenario": "S0"}, {"value": "0", "module": "C4", "scenario": "S1"}, {"value": "0.000411686353632979", "module": "C4", "scenario": "S2"}, {"value": "-0.00462404796200714", "module": "D", "scenario": "S0"}, {"value": "-0.00466283740539496", "module": "D", "scenario": "S1"}, {"value": "0", "module": "D", "scenario": "S2"}]}}, {"referenceToLCIAMethodDataSet": {"shortDescription": [{"value": "Bildungspotential für troposphärisches Ozon (POCP)", "lang": "de"}, {"value": "Formation potential of tropospheric ozone photochemical oxidants (POCP)", "lang": "en"}], "type": "LCIA method data set", "refObjectId": "b5c610fe-def3-11e6-bf01-fe55135034f3", "uri": "../lciamethods/b5c610fe-def3-11e6-bf01-fe55135034f3.xml"}, "other": {"anies": [{"name": "referenceToUnitGroupDataSet", "value": {"shortDescription": [{"value": "kg NMVOC-Äq.", "lang": "de"}], "type": "unit group data set", "refObjectId": "d27c25f8-fbc1-44c6-b47b-4adbae4199c6", "uri": "../unitgroups/d27c25f8-fbc1-44c6-b47b-4adbae4199c6.xml"}}, {"value": "0.00287866919394666", "module": "A1-A3"}, {"value": "0.000179803167679468", "module": "A4"}, {"value": "0.000109444654374272", "module": "A5"}, {"value": "4.17400999995579E-05", "module": "C1"}, {"value": "1.06173075503075E-05", "module": "C2", "scenario": "S0"}, {"value": "3.00593902073642E-05", "module": "C2", "scenario": "S1"}, {"value": "1.06173075503075E-05", "module": "C2", "scenario": "S2"}, {"value": "0.000197615255706475", "module": "C3", "scenario": "S0"}, {"value": "0.00028424593577791", "module": "C3", "scenario": "S1"}, {"value": "0", "module": "C3", "scenario": "S2"}, {"value": "0", "module": "C4", "scenario": "S0"}, {"value": "0", "module": "C4", "scenario": "S1"}, {"value": "0.000120024188794085", "module": "C4", "scenario": "S2"}, {"value": "-0.00122002150608816", "module": "D", "scenario": "S0"}, {"value": "-0.00194675850118751", "module": "D", "scenario": "S1"}, {"value": "0", "module": "D", "scenario": "S2"}]}}, {"referenceToLCIAMethodDataSet": {"shortDescription": [{"value": "Potenzial für den abiotischen Abbau nicht fossiler Ressourcen (ADPE)", "lang": "de"}, {"value": "Abiotic depletion potential for non fossil resources (ADPE)", "lang": "en"}], "type": "LCIA method data set", "refObjectId": "b2ad6494-c78d-11e6-9d9d-cec0c932ce01", "uri": "../lciamethods/b2ad6494-c78d-11e6-9d9d-cec0c932ce01.xml"}, "other": {"anies": [{"name": "referenceToUnitGroupDataSet", "value": {"shortDescription": [{"value": "kg Sb-Äq.", "lang": "de"}], "type": "unit group data set", "refObjectId": "54ccd2d9-a32a-4fc2-923d-f2c8c93e89d4", "uri": "../unitgroups/54ccd2d9-a32a-4fc2-923d-f2c8c93e89d4.xml"}}, {"value": "1.49442096195675E-07", "module": "A1-A3"}, {"value": "7.29541249304767E-09", "module": "A4"}, {"value": "1.22415849211448E-09", "module": "A5"}, {"value": "5.03260114418398E-10", "module": "C1"}, {"value": "5.93177486105544E-10", "module": "C2", "scenario": "S0"}, {"value": "1.6793856100131E-09", "module": "C2", "scenario": "S1"}, {"value": "5.93177486105544E-10", "module": "C2", "scenario": "S2"}, {"value": "1.7075552969042E-09", "module": "C3", "scenario": "S0"}, {"value": "3.4283742985652E-09", "module": "C3", "scenario": "S1"}, {"value": "0", "module": "C3", "scenario": "S2"}, {"value": "0", "module": "C4", "scenario": "S0"}, {"value": "0", "module": "C4", "scenario": "S1"}, {"value": "1.93379085335335E-09", "module": "C4", "scenario": "S2"}, {"value": "-1.16523041832302E-07", "module": "D", "scenario": "S0"}, {"value": "-5.41515445226298E-08", "module": "D", "scenario": "S1"}, {"value": "0", "module": "D", "scenario": "S2"}]}}, {"referenceToLCIAMethodDataSet": {"shortDescription": [{"value": "Potenzial für den abiotischen Abbau fossiler Brennstoffe (ADPF)", "lang": "de"}, {"value": "Abiotic depletion potential for fossil resources (ADPF)", "lang": "en"}], "type": "LCIA method data set", "refObjectId": "b2ad6110-c78d-11e6-9d9d-cec0c932ce01", "uri": "../lciamethods/b2ad6110-c78d-11e6-9d9d-cec0c932ce01.xml"}, "other": {"anies": [{"name": "referenceToUnitGroupDataSet", "value": {"shortDescription": [{"value": "MJ", "lang": "de"}], "type": "unit group data set", "refObjectId": "93a60a57-a3c8-11da-a746-0800200c9a66", "uri": "../unitgroups/93a60a57-a3c8-11da-a746-0800200c9a66.xml"}}, {"value": "55.3254638453613", "module": "A1-A3"}, {"value": "1.10329700264546", "module": "A4"}, {"value": "0.701502646450007", "module": "A5"}, {"value": "0.564517126454692", "module": "C1"}, {"value": "0.0897071883297473", "module": "C2", "scenario": "S0"}, {"value": "0.253976195530973", "module": "C2", "scenario": "S1"}, {"value": "0.0897071883297473", "module": "C2", "scenario": "S2"}, {"value": "0.358115897912899", "module": "C3", "scenario": "S0"}, {"value": "3.72449346580009", "module": "C3", "scenario": "S1"}, {"value": "0", "module": "C3", "scenario": "S2"}, {"value": "0", "module": "C4", "scenario": "S0"}, {"value": "0", "module": "C4", "scenario": "S1"}, {"value": "0.491578890493222", "module": "C4", "scenario": "S2"}, {"value": "-24.0244267553844", "module": "D", "scenario": "S0"}, {"value": "-24.2883195641801", "module": "D", "scenario": "S1"}, {"value": "0", "module": "D", "scenario": "S2"}]}}, {"referenceToLCIAMethodDataSet": {"shortDescription": [{"value": "Wassernutzung (WDP)", "lang": "de"}, {"value": "Water use (WDP)", "lang": "en"}], "type": "LCIA method data set", "refObjectId": "b2ad66ce-c78d-11e6-9d9d-cec0c932ce01", "uri": "../lciamethods/b2ad66ce-c78d-11e6-9d9d-cec0c932ce01.xml"}, "other": {"anies": [{"name": "referenceToUnitGroupDataSet", "value": {"shortDescription": [{"value": "m^(3) Welt-Äq. entzogen", "lang": "de"}], "type": "unit group data set", "refObjectId": "6ae2df01-888e-46c8-b17d-49fa3869b476", "uri": "../unitgroups/6ae2df01-888e-46c8-b17d-49fa3869b476.xml"}}, {"value": "0.00753263224457257", "module": "A1-A3"}, {"value": "0.00129709333837198", "module": "A4"}, {"value": "0.0196634768803907", "module": "A5"}, {"value": "0.00321532246651235", "module": "C1"}, {"value": "0.000105464436237557", "module": "C2", "scenario": "S0"}, {"value": "0.000298587624672574", "module": "C2", "scenario": "S1"}, {"value": "0.000105464436237557", "module": "C2", "scenario": "S2"}, {"value": "0.286061239950716", "module": "C3", "scenario": "S0"}, {"value": "0.0992497630358358", "module": "C3", "scenario": "S1"}, {"value": "0", "module": "C3", "scenario": "S2"}, {"value": "0", "module": "C4", "scenario": "S0"}, {"value": "0", "module": "C4", "scenario": "S1"}, {"value": "0.00375989055196424", "module": "C4", "scenario": "S2"}, {"value": "-0.144353774368724", "module": "D", "scenario": "S0"}, {"value": "-0.108986215739407", "module": "D", "scenario": "S1"}, {"value": "0", "module": "D", "scenario": "S2"}]}}, {"referenceToLCIAMethodDataSet": {"shortDescription": [{"value": "Auftreten von Krankheiten aufgrund von Feinstaubemissionen (PM)", "lang": "de"}, {"value": "Incidence of disease due to PM emissions (PM)", "lang": "en"}], "type": "LCIA method data set", "refObjectId": "b5c602c6-def3-11e6-bf01-fe55135034f3", "uri": "../lciamethods/b5c602c6-def3-11e6-bf01-fe55135034f3.xml"}, "other": {"anies": [{"name": "referenceToUnitGroupDataSet", "value": {"shortDescription": [{"value": "Krankheitsfälle", "lang": "de"}], "type": "unit group data set", "refObjectId": "3883559b-648f-4afc-8ba2-0bd24f3affa3", "uri": "../unitgroups/3883559b-648f-4afc-8ba2-0bd24f3affa3.xml"}}, {"value": "2.80944898210618E-08", "module": "A1-A3"}, {"value": "1.51345556177087E-09", "module": "A4"}, {"value": "9.25177194360749E-10", "module": "A5"}, {"value": "5.03263308816389E-10", "module": "C1"}, {"value": "1.12716719002177E-10", "module": "C2", "scenario": "S0"}, {"value": "3.1912006159058E-10", "module": "C2", "scenario": "S1"}, {"value": "1.12716719002177E-10", "module": "C2", "scenario": "S2"}, {"value": "1.80265785860197E-09", "module": "C3", "scenario": "S0"}, {"value": "3.39931067699255E-09", "module": "C3", "scenario": "S1"}, {"value": "0", "module": "C3", "scenario": "S2"}, {"value": "0", "module": "C4", "scenario": "S0"}, {"value": "0", "module": "C4", "scenario": "S1"}, {"value": "1.80343459953219E-09", "module": "C4", "scenario": "S2"}, {"value": "-1.15475823972542E-08", "module": "D", "scenario": "S0"}, {"value": "-1.17782772317382E-08", "module": "D", "scenario": "S1"}, {"value": "0", "module": "D", "scenario": "S2"}]}}, {"referenceToLCIAMethodDataSet": {"shortDescription": [{"value": "Wirkung durch Exposition des Menschen mit U235 (IR)", "lang": "de"}, {"value": "Human exposure efficiency relative to U235 (IR)", "lang": "en"}], "type": "LCIA method data set", "refObjectId": "b5c632be-def3-11e6-bf01-fe55135034f3", "uri": "../lciamethods/b5c632be-def3-11e6-bf01-fe55135034f3.xml"}, "other": {"anies": [{"name": "referenceToUnitGroupDataSet", "value": {"shortDescription": [{"value": "kBq U235-Äq.", "lang": "de"}], "type": "unit group data set", "refObjectId": "456b05bf-1415-44a9-9993-02452f554c09", "uri": "../unitgroups/456b05bf-1415-44a9-9993-02452f554c09.xml"}}, {"value": "0.0235967908535542", "module": "A1-A3"}, {"value": "0.000291507189970335", "module": "A4"}, {"value": "0.00570208186501143", "module": "A5"}, {"value": "0.00422252429043887", "module": "C1"}, {"value": "2.37019499984515E-05", "module": "C2", "scenario": "S0"}, {"value": "6.71042220735381E-05", "module": "C2", "scenario": "S1"}, {"value": "2.37019499984515E-05", "module": "C2", "scenario": "S2"}, {"value": "0.00329266879774139", "module": "C3", "scenario": "S0"}, {"value": "0.0278423140489482", "module": "C3", "scenario": "S1"}, {"value": "0", "module": "C3", "scenario": "S2"}, {"value": "0", "module": "C4", "scenario": "S0"}, {"value": "0", "module": "C4", "scenario": "S1"}, {"value": "0.000950926132794427", "module": "C4", "scenario": "S2"}, {"value": "-0.289874494033189", "module": "D", "scenario": "S0"}, {"value": "-0.0412848262988982", "module": "D", "scenario": "S1"}, {"value": "0", "module": "D", "scenario": "S2"}]}}, {"referenceToLCIAMethodDataSet": {"shortDescription": [{"value": "Toxizitätsvergleichseinheit für Ökosysteme (ETP-fw)", "lang": "de"}, {"value": "Comparative toxic unit for ecosystems (ETP-fw)", "lang": "en"}], "type": "LCIA method data set", "refObjectId": "ee1082d1-b0f7-43ca-a1f0-21e2a4a74511", "uri": "../lciamethods/ee1082d1-b0f7-43ca-a1f0-21e2a4a74511.xml"}, "other": {"anies": [{"name": "referenceToUnitGroupDataSet", "value": {"shortDescription": [{"value": "CTUe", "lang": "de"}], "type": "unit group data set", "refObjectId": "aa959ded-f1eb-4efb-9c5c-2d60be36b3e6", "uri": "../unitgroups/aa959ded-f1eb-4efb-9c5c-2d60be36b3e6.xml"}}, {"value": "26.9419111137323", "module": "A1-A3"}, {"value": "0.819072622770789", "module": "A4"}, {"value": "0.516753933822934", "module": "A5"}, {"value": "0.0789851067987469", "module": "C1"}, {"value": "0.0665967365789065", "module": "C2", "scenario": "S0"}, {"value": "0.188546604859761", "module": "C2", "scenario": "S1"}, {"value": "0.0665967365789065", "module": "C2", "scenario": "S2"}, {"value": "0.14796773693347", "module": "C3", "scenario": "S0"}, {"value": "0.530405129949021", "module": "C3", "scenario": "S1"}, {"value": "0", "module": "C3", "scenario": "S2"}, {"value": "0", "module": "C4", "scenario": "S0"}, {"value": "0", "module": "C4", "scenario": "S1"}, {"value": "1.0650931070489", "module": "C4", "scenario": "S2"}, {"value": "-3.38049136376811", "module": "D", "scenario": "S0"}, {"value": "-12.7958030791417", "module": "D", "scenario": "S1"}, {"value": "0", "module": "D", "scenario": "S2"}]}}, {"referenceToLCIAMethodDataSet": {"shortDescription": [{"value": "Toxizitätsvergleichseinheit für Menschen (krebserregend) (HTP-c)", "lang": "de"}, {"value": "Comparative toxic unit for humans (carcinogenic) (HTP-c)", "lang": "en"}], "type": "LCIA method data set", "refObjectId": "2299222a-bbd8-474f-9d4f-4dd1f18aea7c", "uri": "../lciamethods/2299222a-bbd8-474f-9d4f-4dd1f18aea7c.xml"}, "other": {"anies": [{"name": "referenceToUnitGroupDataSet", "value": {"shortDescription": [{"value": "CTUh", "lang": "de"}], "type": "unit group data set", "refObjectId": "d4c9523e-2d7e-49fd-8469-998f547d3a70", "uri": "../unitgroups/d4c9523e-2d7e-49fd-8469-998f547d3a70.xml"}}, {"value": "6.97233261390834E-10", "module": "A1-A3"}, {"value": "1.65454771044438E-11", "module": "A4"}, {"value": "5.703818749123E-11", "module": "A5"}, {"value": "3.17117107548698E-12", "module": "C1"}, {"value": "1.3445488561959E-12", "module": "C2", "scenario": "S0"}, {"value": "3.80664481364554E-12", "module": "C2", "scenario": "S1"}, {"value": "1.3445488561959E-12", "module": "C2", "scenario": "S2"}, {"value": "2.01990655462407E-11", "module": "C3", "scenario": "S0"}, {"value": "2.1978333013805E-11", "module": "C3", "scenario": "S1"}, {"value": "0", "module": "C3", "scenario": "S2"}, {"value": "0", "module": "C4", "scenario": "S0"}, {"value": "0", "module": "C4", "scenario": "S1"}, {"value": "1.57968142304033E-11", "module": "C4", "scenario": "S2"}, {"value": "-2.74752472224489E-10", "module": "D", "scenario": "S0"}, {"value": "-2.97573979250827E-10", "module": "D", "scenario": "S1"}, {"value": "0", "module": "D", "scenario": "S2"}]}}, {"referenceToLCIAMethodDataSet": {"shortDescription": [{"value": "Toxizitätsvergleichseinheit für Menschen (nicht krebserregend) (HTP-nc)", "lang": "de"}, {"value": "Comparative toxic unit for humans (noncarcinogenic) (HTP-nc)", "lang": "en"}], "type": "LCIA method data set", "refObjectId": "3af763a5-b7a1-48c9-9cee-1f223481fcef", "uri": "../lciamethods/3af763a5-b7a1-48c9-9cee-1f223481fcef.xml"}, "other": {"anies": [{"name": "referenceToUnitGroupDataSet", "value": {"shortDescription": [{"value": "CTUh", "lang": "de"}], "type": "unit group data set", "refObjectId": "d4c9523e-2d7e-49fd-8469-998f547d3a70", "uri": "../unitgroups/d4c9523e-2d7e-49fd-8469-998f547d3a70.xml"}}, {"value": "2.63130858744598E-08", "module": "A1-A3"}, {"value": "7.42457756559675E-10", "module": "A4"}, {"value": "5.39778958509947E-09", "module": "A5"}, {"value": "1.22346483313125E-10", "module": "C1"}, {"value": "6.03574691657462E-11", "module": "C2", "scenario": "S0"}, {"value": "1.70882185430294E-10", "module": "C2", "scenario": "S1"}, {"value": "6.03574691657462E-11", "module": "C2", "scenario": "S2"}, {"value": "1.32783947668853E-10", "module": "C3", "scenario": "S0"}, {"value": "8.20852021740948E-10", "module": "C3", "scenario": "S1"}, {"value": "0", "module": "C3", "scenario": "S2"}, {"value": "0", "module": "C4", "scenario": "S0"}, {"value": "0", "module": "C4", "scenario": "S1"}, {"value": "3.30726185157412E-10", "module": "C4", "scenario": "S2"}, {"value": "-6.46149638731735E-09", "module": "D", "scenario": "S0"}, {"value": "-9.28104126631768E-09", "module": "D", "scenario": "S1"}, {"value": "0", "module": "D", "scenario": "S2"}]}}, {"referenceToLCIAMethodDataSet": {"shortDescription": [{"value": "Bodenqualitätsindex (SQP)", "lang": "de"}, {"value": "Soil quality index (SQP)", "lang": "en"}], "type": "LCIA method data set", "refObjectId": "b2ad6890-c78d-11e6-9d9d-cec0c932ce01", "uri": "../lciamethods/b2ad6890-c78d-11e6-9d9d-cec0c932ce01.xml"}, "other": {"anies": [{"name": "referenceToUnitGroupDataSet", "value": {"shortDescription": [{"value": "SQP", "lang": "de"}], "type": "unit group data set", "refObjectId": "f130951c-e67f-4f7f-8dd4-665de3974e18", "uri": "../unitgroups/f130951c-e67f-4f7f-8dd4-665de3974e18.xml"}}, {"value": "22.2393336750675", "module": "A1-A3"}, {"value": "0.542670461807416", "module": "A4"}, {"value": "0.0902411117129215", "module": "A5"}, {"value": "0.0481641618822683", "module": "C1"}, {"value": "0.0441236051594636", "module": "C2", "scenario": "S0"}, {"value": "0.124921375646274", "module": "C2", "scenario": "S1"}, {"value": "0.0441236051594636", "module": "C2", "scenario": "S2"}, {"value": "0.116259317158171", "module": "C3", "scenario": "S0"}, {"value": "0.32454298071918", "module": "C3", "scenario": "S1"}, {"value": "0", "module": "C3", "scenario": "S2"}, {"value": "0", "module": "C4", "scenario": "S0"}, {"value": "0", "module": "C4", "scenario": "S1"}, {"value": "0.0834938587686752", "module": "C4", "scenario": "S2"}, {"value": "-4.69438544231198", "module": "D", "scenario": "S0"}, {"value": "-0.713918113263341", "module": "D", "scenario": "S1"}, {"value": "0", "module": "D", "scenario": "S2"}]}}]}, "otherAttributes": {"{http://www.indata.network/EPD/2019}epd-version": "1.2"}, "version": "1.1", "locations": "../ILCDLocations.xml"}