{"processInformation": {"dataSetInformation": {"UUID": "b144ce25-34af-437d-b324-1dfdcb20a889", "name": {"baseName": [{"value": "Cementex/Cementex Extreme", "lang": "en"}, {"value": "Cementex/Cementex Extreme", "lang": "de"}], "functionalUnitFlowProperties": [{"lang": "en"}]}, "classificationInformation": {"classification": [{"class": [{"value": "Mineralische Baustoffe", "level": 0, "classId": "1"}, {"value": "Steine und Elemente", "level": 1, "classId": "1.3"}, {"value": "Faserzement", "level": 2, "classId": "1.3.12"}], "name": "OEKOBAU.DAT"}, {"class": [{"value": "02 Building products", "level": 0}, {"value": "Facades", "level": 1}, {"value": "Fibre cement / Fibre concrete", "level": 2}], "name": "IBUCategories"}]}, "generalComment": [{"value": "Cementex and Cementex Extreme are cellulose reinforced fibre cement boards. The main difference between the products is that Cementex Extreme has an additional hydrophobic layer.\n\nCementex / Cementex Extreme boards are highly durable and suitable for external and internal applications. The boards are manufactured using the Hatschek technology and then autoclaved, which ensures optimal dimensional stability and mechanical resistance. The boards are available with squared edges.", "lang": "en"}], "other": {"anies": [{"scenario": [{"description": [{"value": "100% Landfill", "lang": "en"}, {"value": "100% Deponierung", "lang": "de"}], "name": "S0", "default": true}, {"description": [{"value": "Scenario 1", "lang": "en"}, {"value": "Szenario 1", "lang": "de"}], "name": "S1"}, {"description": [{"value": "Scenario 2", "lang": "en"}, {"value": "Szenario 2", "lang": "de"}], "name": "S2"}, {"description": [{"value": "Scenario 3", "lang": "en"}, {"value": "Szenario 3", "lang": "de"}], "name": "S3"}]}]}}, "quantitativeReference": {"referenceToReferenceFlow": [0]}, "time": {"referenceYear": 2022, "dataSetValidUntil": 2027, "other": {"anies": [{"name": "publicationDateOfEPD", "value": 1666569600000}]}}, "geography": {"locationOfOperationSupplyOrProduction": {"location": "RER"}}, "technology": {"technologyDescriptionAndIncludedProcesses": [{"value": "Cementex fibre cement boards are manufactured largely in accordance to an automated winding process, the Hatschek process: the raw materials are mixed with water to prepare a homogenous mixture. Rotating screen cylinders are immersed in this fiber cement pulp which drain internally. The screen surface is covered in a thin film of fiber cement which is transferred onto an infinite conveyor belt from where it is conveyed to a format roller or forming drum which is gradually covered in an increasingly thicker layer of fiber cement. Once the requisite material thickness is achieved, the still moist and malleable fiber cement layer (fiber cement fleece) is separated and removed from the forming drum. The fiber cement fleece is cut to size. Leftovers are returned to the production process preventing any waste from being incurred. The sheets are then laid on templates, and steam-hardened in an autoclave. The Cementex boards are then calibrated, sanded and for the Cementex Extreme boards, a hydrophobation layer is applied at both sides. Base materials/Ancillary materials Main raw materials used (in weight percentages): Portland Cement - 25-45% Sand M32 - 35-50% Cellulose - <10% others - <10% \nTechnical data: \nThe safety of a building is directly linked to the quality of the materials employed in its construction. The use of standardized materials and proper handling procedures is one of the ways construction industries ensure a building’s safety.\n\nEtex on-site laboratories perform chemical and mechanical tests guaranteeing compliance of the final products to technical standard requirements. Technical product specification is set by European standard EN 12467:2013 + A2:2018 ‘Fibre-cement flat sheets’. \nDeclared unit: \nThe functional unit is 1 m2 of Cementex / Cementex Extreme of 10 mm thickness.", "lang": "en"}, {"value": "Cementex Faserzementplatten werden weitgehend nach einem automatisierten Wickelverfahren, dem Hatschek-Verfahren, hergestellt: Die Rohstoffe werden mit Wasser zu einem homogenen Gemisch vermischt. In diesen Faserzementbrei werden rotierende Siebzylinder eingetaucht, die im Inneren entwässern. Die Sieboberfläche wird mit einem dünnen Film aus Faserzement bedeckt, der auf ein endloses Förderband übertragen wird, von wo aus er zu einer Formatwalze oder Formtrommel befördert wird, die nach und nach mit einer immer dickeren Schicht aus Faserzement bedeckt wird. Ist die erforderliche Materialdicke erreicht, wird die noch feuchte und verformbare Faserzementschicht (Faserzementvlies) abgetrennt und von der Formtrommel entfernt. Das Faserzementvlies wird auf Maß geschnitten. Die Reste werden in den Produktionsprozess zurückgeführt, so dass kein Abfall anfällt. Die Platten werden dann auf Schablonen gelegt und in einem Autoklaven dampfgehärtet. Die Cementex-Platten werden dann kalibriert, geschliffen und bei den Cementex Extreme-Platten beidseitig mit einer Hydrophobierungsschicht versehen.\n\n\n\nGrundstoffe/Hilfsstoffe\n\nVerwendete Hauptrohstoffe (in Gewichtsprozenten):\n\nPortlandzement - 25-45%\n\nSand M32 - 35-50%\n\nZellulose - <10%\n\nandere - <10% \n", "lang": "de"}], "technologicalApplicability": [{"value": "The Cementex / Cementex Extreme boards are suitable for internal and external applications.\n\nInner wall: non-load-bearing partition wall, retaining wall, timber frame wall, steel frame wall.\nInterior floor: finishing backer and loadbearing plate on load-bearing floors and floating floors\nInterior ceiling: suspended ceilings, pool ceilings\nOutdoor: wall and ceiling cladding in the not directly exposed outdoor area.\n\nManufacturing Process\n\n\nCementex fibre cement boards are manufactured largely in accordance with an automated winding process, the Hatschek process: the raw materials are mixed with water to prepare a homogenous mixture. Rotating screen cylinders are immersed in this fibre cement pulp which drains internally. The screen surface is covered in a thin film of fibre cement which is transferred onto an infinite conveyor belt from where it is conveyed to a format roller or forming drum which is gradually covered in an increasingly thicker layer of fibre cement. Once the requisite material thickness is achieved, the still moist and malleable fibre cement layer (fibre cement fleece) is separated and removed from the forming drum. The fibre cement fleece is cut to size. Leftovers are returned to the production process preventing any waste from being incurred. The sheets are then laid on templates and steam-hardened in an autoclave. The Cementex boards are then calibrated, sanded and for the Cementex Extreme boards, a hydrophobic layer is applied at both sides.\n\n\nThe quality management system of the production facilities is certified according to ISO 9001;2015.\n\nInstallation\n\nThe Cementex / Cementex Extreme boards are mainly fixed with screws on a metal or wooden substructure. The joints are treated with a jointing compound, a reinforcement tape is used over the edges and the boards are finished with a finishing compound. \n\n Environment and health during manufacturing\n\nEnvironmental, occupational health and safety management system at the Cementex production plants are in accordance with the following standards:\n\nISO 14001;2015\n\nISO 45001;2018\n\n\nCondition of use\n\nMaintenance requirement will depend on the specific design and application. Usually Cementex / Cementex Extreme won’t change the composition of the materials and thus no maintenance is needed.\n\n\nEnvironment and health during use\n\nWhen the boards are used as designed, the current state of knowledge indicates that there is no risk involved for the environment or health.\n\n\nWater\n\nAll ingredients are firmly bound in the matrix. The boards are insensitive to moisture and no ingredients which could be hazardous to water are expected to be washed out in the event of extraordinary effects by water.\n\n\nMechanical destruction\n\n\nIn case of mechanical destruction, no risks are expected to occur in terms of environment and human health.", "lang": "en"}, {"value": "Die Cementex / Cementex Extreme Platten sind für Innen- und Außenanwendungen geeignet.\n\n\n\nInnenwand: nicht tragende Trennwand, Stützwand, Holzrahmenwand, Stahlrahmenwand.\nInnenboden: Abschluss- und Tragplatte auf tragenden und schwimmenden Böden\nInnendecke: abgehängte Decken, Pool-Decken\nAußenbereich: Wand- und Deckenverkleidungen im nicht direkt exponierten Außenbereich.\nHerstellungsverfahren\n\nCementex Faserzementplatten werden weitgehend nach einem automatisierten Wickelverfahren, dem Hatschek-Verfahren, hergestellt: Die Rohstoffe werden mit Wasser zu einem homogenen Gemisch vermischt. Rotierende Siebzylinder werden in diesen Faserzementbrei getaucht, der im Inneren abläuft. Die Sieboberfläche wird mit einem dünnen Film aus Faserzement überzogen, der auf ein endloses Förderband übertragen wird, von wo aus er zu einer Formatwalze oder Formtrommel befördert wird, die nach und nach mit einer immer dickeren Schicht Faserzement überzogen wird. Ist die erforderliche Materialdicke erreicht, wird die noch feuchte und verformbare Faserzementschicht (Faserzementvlies) abgetrennt und von der Formtrommel entfernt. Das Faserzementvlies wird auf Maß geschnitten. Reste werden in den Produktionsprozess zurückgeführt, so dass keine Abfälle anfallen. Die Platten werden dann auf Schablonen gelegt und in einem Autoklaven dampfgehärtet. Die Cementex-Platten werden dann kalibriert, geschliffen und bei den Cementex Extreme-Platten beidseitig mit einer hydrophoben Schicht versehen.\n\n\n\nDas Qualitätsmanagementsystem der Produktionsanlagen ist nach ISO 9001;2015 zertifiziert.\n\n \n\n \n\nVerlegung\n\nDie Cementex / Cementex Extreme Platten werden hauptsächlich mit Schrauben auf einer Metall- oder Holzunterkonstruktion befestigt. Die Fugen werden mit einer Fugenmasse behandelt, an den Kanten wird ein Verstärkungsband verwendet und die Platten werden mit einer Endbearbeitungsmasse fertiggestellt. \n\n\nUmwelt und Gesundheit bei der Herstellung\n\nDas Umwelt-, Arbeitsschutz- und Sicherheitsmanagementsystem in den Cementex-Produktionsstätten entspricht den folgenden Normen:\n\nISO 14001;2015\n\nISO 45001; 2018\n\n \n\nZustand der Nutzung\n\nDer Wartungsbedarf hängt von der spezifischen Konstruktion und Anwendung ab. Normalerweise verändert Cementex / Cementex Extreme die Zusammensetzung der Materialien nicht, so dass keine Wartung erforderlich ist.\n\n \n\nUmwelt und Gesundheit während der Nutzung\n\nWenn die Platten wie vorgesehen verwendet werden, besteht nach derzeitigem Kenntnisstand kein Risiko für die Umwelt oder die Gesundheit.\n\n \n\nWasser\n\nAlle Inhaltsstoffe sind fest in der Matrix gebunden. Die Platten sind feuchtigkeitsunempfindlich und es sind keine wassergefährdenden Inhaltsstoffe zu erwarten, die bei außergewöhnlichen Einwirkungen durch Wasser ausgewaschen werden könnten.\n\n \n\nMechanische Zerstörung\n\nBei mechanischer Zerstörung sind keine Risiken für die Umwelt und die menschliche Gesundheit zu erwarten.", "lang": "de"}]}}, "modellingAndValidation": {"LCIMethodAndAllocation": {"typeOfDataSet": "EPD", "referenceToLCAMethodDetails": [{"shortDescription": [{"value": "Fibre cement / Fibre concrete.pdf", "lang": "en"}], "type": "source data set", "refObjectId": "cd340094-5110-4728-9e08-cda963239c03"}], "other": {"anies": [{"name": "subType", "value": "specific dataset"}]}}, "dataSourcesTreatmentAndRepresentativeness": {"referenceToDataSource": [{"shortDescription": [{"value": "ecoinvent database (all versions)", "lang": "en"}], "type": "source data set", "refObjectId": "b497a91f-e14b-4b69-8f28-f50eb1576766"}, {"shortDescription": [{"value": "ecoinvent 3.6 database", "lang": "en"}], "type": "source data set", "refObjectId": "766b9973-5ee8-48a2-8098-72c8e20b369f"}], "useAdviceForDataSet": [{"value": "Scope: \nThe life cycle assessment is based on the production data of Cementex / Cementex Extreme of the year 2019 at the two Etex production sites in Gresik and Karawang, both located in Indonesia. The average of the data collected from both plants has been used in this LCA study. \nSystem boundary: \nThis study takes into account the mandatory life cycle stages of the EN15804+A2 for a cradle-to-grave LCA study, being modules A1, A2, A3, A4, A5, B1, B2, B3, B4, B5, B6, B7, C1, C2, C3, C4 and D.\n\nLife cycle stages:\n\nProduct stage: production of raw materials (A1), transport of raw materials to manufacturing site (A2), production of final product (A3);\nConstruction process stage: transport to construction site (A4), construction/installation process (A5);\nUse stage: use (B1), maintenance (B2), repair (B3), replacements (B4), refurbishment (B5), operational energy use (B6), operational water use (B7);\nEnd-of-life stage: deconstruction/demolition (C1), transport to end-of-life treatment (C2), waste processing (C3) and final disposal (C4)\nBenefits and loads beyond the system boundaries: reuse, recovery, recycling potential (D)", "lang": "en"}], "other": {"anies": [{"name": "referenceToOriginalEPD", "value": {"shortDescription": {"value": "Cementex/Cementex Extreme.pdf", "defaultValue": "Cementex/Cementex Extreme.pdf", "lstrings": [{"lang": "en", "value": "Cementex/Cementex Extreme.pdf"}]}, "type": "source data set", "uuid": {"uuid": "0a2d7a4e-0cc8-4a21-a67c-1a4a760d3411"}, "refObjectId": "0a2d7a4e-0cc8-4a21-a67c-1a4a760d3411", "resourceURLs": ["https://oekobaudat.de/OEKOBAU.DAT/resource/sources/0a2d7a4e-0cc8-4a21-a67c-1a4a760d3411/CementexCementex_Extreme_15991.pdf?version=00.01.000"]}}]}}, "validation": {"review": [{"referenceToNameOfReviewerAndInstitution": [{"shortDescription": [{"value": "Institut Bauen und Umwelt e. V.", "lang": "en"}], "type": "contact data set", "refObjectId": "d111dbec-b024-4be5-86c5-752d6eb2cf95", "uri": "../contacts/d111dbec-b024-4be5-86c5-752d6eb2cf95.xml"}], "type": "Accredited third party review"}]}, "complianceDeclarations": {"compliance": [{"referenceToComplianceSystem": {"shortDescription": [{"value": "DIN EN 15804+A2", "lang": "en"}], "type": "source data set", "refObjectId": "c0016b33-8cf7-415c-ac6e-deba0d21440d", "uri": "../sources/c0016b33-8cf7-415c-ac6e-deba0d21440d.xml"}}, {"referenceToComplianceSystem": {"shortDescription": [{"value": "ISO 14025", "lang": "en"}], "type": "source data set", "refObjectId": "4f2eb655-6e44-4874-a95a-e28f5442cd4d", "uri": "../sources/4f2eb655-6e44-4874-a95a-e28f5442cd4d.xml"}}]}}, "administrativeInformation": {"commissionerAndGoal": {"referenceToCommissioner": [{"shortDescription": [{"value": "Etex Building Performance International", "lang": "en"}], "type": "contact data set", "refObjectId": "9f15c029-1fb0-467d-8dd1-92b013e91ca8", "uri": "../contacts/9f15c029-1fb0-467d-8dd1-92b013e91ca8.xml"}]}, "dataGenerator": {"referenceToPersonOrEntityGeneratingTheDataSet": [{"shortDescription": [{"value": "Etex Building Performance International", "lang": "en"}], "type": "contact data set", "refObjectId": "9f15c029-1fb0-467d-8dd1-92b013e91ca8", "uri": "../contacts/9f15c029-1fb0-467d-8dd1-92b013e91ca8.xml"}]}, "dataEntryBy": {"timeStamp": 1666610999459, "referenceToDataSetFormat": [{"shortDescription": [{"value": "ILCD Format", "lang": "en"}], "type": "source data set", "refObjectId": "a97a0155-0234-4b87-b4ce-a45da52f2a40", "uri": "../sources/a97a0155-0234-4b87-b4ce-a45da52f2a40.xml"}, {"shortDescription": [{"value": "EPD-Datenformaterweiterungen v1.2", "lang": "de"}, {"value": "EPD Data Format Extensions v1.2", "lang": "en"}], "type": "source data set", "refObjectId": "a29449fd-aa2f-4de8-b5d7-4b06b43c6fde", "uri": "../sources/a29449fd-aa2f-4de8-b5d7-4b06b43c6fde.xml"}]}, "publicationAndOwnership": {"dataSetVersion": "00.01.000", "referenceToRegistrationAuthority": {"shortDescription": [{"value": "Institut Bauen und Umwelt e. V.", "lang": "en"}], "type": "contact data set", "refObjectId": "d111dbec-b024-4be5-86c5-752d6eb2cf95", "uri": "../contacts/d111dbec-b024-4be5-86c5-752d6eb2cf95.xml"}, "registrationNumber": "EPD-ETE-20220212-CCA1-EN", "referenceToOwnershipOfDataSet": {"shortDescription": [{"value": "Etex Building Performance International", "lang": "en"}], "type": "contact data set", "refObjectId": "9f15c029-1fb0-467d-8dd1-92b013e91ca8", "uri": "../contacts/9f15c029-1fb0-467d-8dd1-92b013e91ca8.xml"}, "copyright": true, "licenseType": "Free of charge for all users and uses", "accessRestrictions": [{"value": "None", "lang": "en"}], "other": {"anies": [{"name": "referenceToPublisher", "value": {"shortDescription": [{"value": "Institut Bauen und Umwelt e. V.", "lang": "en"}], "type": "contact data set", "refObjectId": "d111dbec-b024-4be5-86c5-752d6eb2cf95", "uri": "../contacts/d111dbec-b024-4be5-86c5-752d6eb2cf95.xml"}}]}}}, "exchanges": {"exchange": [{"dataSetInternalID": 0, "referenceToFlowDataSet": {"shortDescription": [{"value": "Cementex/Cementex Extreme (10 mm) ()", "lang": "en"}], "type": "flow data set", "refObjectId": "e759cb86-3c1e-0840-ca20-11df0e1f8496", "uri": "../flows/e759cb86-3c1e-0840-ca20-11df0e1f8496.xml"}, "meanAmount": 1.0, "referencesToDataSource": {}, "referenceFlow": true, "resolvedFlowVersion": "00.01.000", "resultingflowAmount": 1.0, "flowProperties": [{"name": [{"lang": "en", "value": "Area"}, {"lang": "de", "value": "Fläche"}], "uuid": "93a60a56-a3c8-19da-a746-0800200c9a66", "referenceFlowProperty": true, "meanValue": 1.0, "referenceUnit": "qm", "unitGroupUUID": "c20a03d7-bd90-4569-bc94-66cfd364dfc8"}], "materialProperties": [{"name": "gross density", "value": "1200.0", "unit": "kg/m^3", "unitDescription": "kilograms per cubic metre"}, {"name": "layer thickness", "value": "0.01", "unit": "m", "unitDescription": "meters"}, {"name": "grammage", "value": "14.6", "unit": "kg/m^2", "unitDescription": "kilograms per square meter"}], "typeOfFlow": "Product flow", "classification": {"classHierarchy": "Mineralische Baustoffe / Steine und Elemente / Faserzement", "name": "OEKOBAU.DAT"}}, {"dataSetInternalID": 1, "referenceToFlowDataSet": {"shortDescription": [{"value": "Renewable primary energy as energy carrier (PERE)", "lang": "en"}, {"value": "Erneuerbare Primärenergie als Energieträger (PERE)", "lang": "de"}], "type": "flow data set", "refObjectId": "20f32be5-0398-4288-9b6d-accddd195317", "uri": "../flows/20f32be5-0398-4288-9b6d-accddd195317.xml"}, "exchange direction": "INPUT", "other": {"anies": [{"name": "referenceToUnitGroupDataSet", "value": {"shortDescription": [{"value": "MJ", "lang": "en"}], "type": "unit group data set", "refObjectId": "93a60a57-a3c8-11da-a746-0800200c9a66", "uri": "../unitgroups/93a60a57-a3c8-11da-a746-0800200c9a66.xml"}}, {"value": "6.73724997176", "module": "A1"}, {"value": "0.1387", "module": "A2"}, {"value": "5.74194241265152", "module": "A3"}, {"value": "0.6471", "module": "A4"}, {"value": "2.45858608062249", "module": "A5"}, {"value": "0", "module": "B1", "scenario": "S1"}, {"value": "0", "module": "B1", "scenario": "S2"}, {"value": "0", "module": "B1", "scenario": "S3"}, {"value": "0", "module": "B2"}, {"value": "0", "module": "B3"}, {"value": "0", "module": "B4"}, {"value": "0", "module": "B5"}, {"value": "0", "module": "B6"}, {"value": "0", "module": "B7"}, {"value": "0.03382", "module": "C1"}, {"value": "0.02655", "module": "C2"}, {"value": "0.0001495", "module": "C3"}, {"value": "0.109", "module": "C4"}, {"value": "0", "module": "D"}]}, "resolvedFlowVersion": "38.00.000", "flowProperties": [], "typeOfFlow": "Other flow", "classification": {"classHierarchy": "Quantities", "name": "GaBiCategories"}}, {"dataSetInternalID": 2, "referenceToFlowDataSet": {"shortDescription": [{"value": "Renewable primary energy resources as material utilization (PERM)", "lang": "en"}, {"value": "Erneuerbare Primärenergie zur stofflichen Nutzung (PERM)", "lang": "de"}], "type": "flow data set", "refObjectId": "fb3ec0de-548d-4508-aea5-00b73bf6f702", "uri": "../flows/fb3ec0de-548d-4508-aea5-00b73bf6f702.xml"}, "exchange direction": "INPUT", "other": {"anies": [{"name": "referenceToUnitGroupDataSet", "value": {"shortDescription": [{"value": "MJ", "lang": "en"}], "type": "unit group data set", "refObjectId": "93a60a57-a3c8-11da-a746-0800200c9a66", "uri": "../unitgroups/93a60a57-a3c8-11da-a746-0800200c9a66.xml"}}, {"value": "15.66215002824", "module": "A1"}, {"value": "0", "module": "A2"}, {"value": "4.38265576952187", "module": "A3"}, {"value": "0", "module": "A4"}, {"value": "-2.69846361022249", "module": "A5"}, {"value": "0", "module": "B1", "scenario": "S1"}, {"value": "0", "module": "B1", "scenario": "S2"}, {"value": "0", "module": "B1", "scenario": "S3"}, {"value": "0", "module": "B2"}, {"value": "0", "module": "B3"}, {"value": "0", "module": "B4"}, {"value": "0", "module": "B5"}, {"value": "0", "module": "B6"}, {"value": "0", "module": "B7"}, {"value": "0", "module": "C1"}, {"value": "0", "module": "C2"}, {"value": "0", "module": "C3"}, {"value": "0", "module": "C4"}, {"value": "1.963892538072", "module": "D"}]}, "resolvedFlowVersion": "38.00.000", "flowProperties": [], "typeOfFlow": "Other flow", "classification": {"classHierarchy": "Quantities", "name": "GaBiCategories"}}, {"dataSetInternalID": 3, "referenceToFlowDataSet": {"shortDescription": [{"value": "Total use of renewable primary energy resources (PERT)", "lang": "en"}, {"value": "Total erneuerbare Primärenergie (PERT)", "lang": "de"}], "type": "flow data set", "refObjectId": "53f97275-fa8a-4cdd-9024-65936002acd0", "uri": "../flows/53f97275-fa8a-4cdd-9024-65936002acd0.xml"}, "exchange direction": "INPUT", "other": {"anies": [{"name": "referenceToUnitGroupDataSet", "value": {"shortDescription": [{"value": "MJ", "lang": "en"}], "type": "unit group data set", "refObjectId": "93a60a57-a3c8-11da-a746-0800200c9a66", "uri": "../unitgroups/93a60a57-a3c8-11da-a746-0800200c9a66.xml"}}, {"value": "22.3994", "module": "A1"}, {"value": "0.1387", "module": "A2"}, {"value": "10.1245981821734", "module": "A3"}, {"value": "0.6471", "module": "A4"}, {"value": "-0.2398775296", "module": "A5"}, {"value": "0", "module": "B1", "scenario": "S1"}, {"value": "0", "module": "B1", "scenario": "S2"}, {"value": "0", "module": "B1", "scenario": "S3"}, {"value": "0", "module": "B2"}, {"value": "0", "module": "B3"}, {"value": "0", "module": "B4"}, {"value": "0", "module": "B5"}, {"value": "0", "module": "B6"}, {"value": "0", "module": "B7"}, {"value": "0.03382", "module": "C1"}, {"value": "0.02655", "module": "C2"}, {"value": "0.0001495", "module": "C3"}, {"value": "0.109", "module": "C4"}, {"value": "1.963892538072", "module": "D"}]}, "resolvedFlowVersion": "38.00.000", "flowProperties": [], "typeOfFlow": "Other flow", "classification": {"classHierarchy": "Quantities / Environmental quantities / EPD EN 15804 / LCI indicators", "name": "GaBiCategories"}}, {"dataSetInternalID": 4, "referenceToFlowDataSet": {"shortDescription": [{"value": "Non renewable primary energy as energy carrier (PENRE)", "lang": "en"}, {"value": "Nicht-erneuerbare Primärenergie als Energieträger (PENRE)", "lang": "de"}], "type": "flow data set", "refObjectId": "ac857178-2b45-46ec-892a-a9a4332f0372", "uri": "../flows/ac857178-2b45-46ec-892a-a9a4332f0372.xml"}, "exchange direction": "INPUT", "other": {"anies": [{"name": "referenceToUnitGroupDataSet", "value": {"shortDescription": [{"value": "MJ", "lang": "en"}], "type": "unit group data set", "refObjectId": "93a60a57-a3c8-11da-a746-0800200c9a66", "uri": "../unitgroups/93a60a57-a3c8-11da-a746-0800200c9a66.xml"}}, {"value": "34.11116512", "module": "A1"}, {"value": "11.67", "module": "A2"}, {"value": "54.42097103552", "module": "A3"}, {"value": "66.45", "module": "A4"}, {"value": "15.973420607776", "module": "A5"}, {"value": "0", "module": "B1", "scenario": "S1"}, {"value": "0", "module": "B1", "scenario": "S2"}, {"value": "0", "module": "B1", "scenario": "S3"}, {"value": "0", "module": "B2"}, {"value": "0", "module": "B3"}, {"value": "0", "module": "B4"}, {"value": "0", "module": "B5"}, {"value": "0", "module": "B6"}, {"value": "0", "module": "B7"}, {"value": "0.2169", "module": "C1"}, {"value": "1.934", "module": "C2"}, {"value": "0.001129", "module": "C3"}, {"value": "2.682", "module": "C4"}, {"value": "0", "module": "D"}]}, "resolvedFlowVersion": "38.00.000", "flowProperties": [], "typeOfFlow": "Other flow", "classification": {"classHierarchy": "Quantities", "name": "GaBiCategories"}}, {"dataSetInternalID": 5, "referenceToFlowDataSet": {"shortDescription": [{"value": "Non renewable primary energy as material utilization (PENRM)", "lang": "en"}, {"value": "Nicht-erneuerbare Primärenergie zur stofflichen Nutzung (PENRM)", "lang": "de"}], "type": "flow data set", "refObjectId": "1421caa0-679d-4bf4-b282-0eb850ccae27", "uri": "../flows/1421caa0-679d-4bf4-b282-0eb850ccae27.xml"}, "exchange direction": "INPUT", "other": {"anies": [{"name": "referenceToUnitGroupDataSet", "value": {"shortDescription": [{"value": "MJ", "lang": "en"}], "type": "unit group data set", "refObjectId": "93a60a57-a3c8-11da-a746-0800200c9a66", "uri": "../unitgroups/93a60a57-a3c8-11da-a746-0800200c9a66.xml"}}, {"value": "0.29883488", "module": "A1"}, {"value": "0", "module": "A2"}, {"value": "0.28906889748", "module": "A3"}, {"value": "0", "module": "A4"}, {"value": "-0.286583607776", "module": "A5"}, {"value": "0", "module": "B1", "scenario": "S1"}, {"value": "0", "module": "B1", "scenario": "S2"}, {"value": "0", "module": "B1", "scenario": "S3"}, {"value": "0", "module": "B2"}, {"value": "0", "module": "B3"}, {"value": "0", "module": "B4"}, {"value": "0", "module": "B5"}, {"value": "0", "module": "B6"}, {"value": "0", "module": "B7"}, {"value": "0", "module": "C1"}, {"value": "0", "module": "C2"}, {"value": "0", "module": "C3"}, {"value": "0", "module": "C4"}, {"value": "0.0365008848", "module": "D"}]}, "resolvedFlowVersion": "38.00.000", "flowProperties": [], "typeOfFlow": "Other flow", "classification": {"classHierarchy": "Quantities", "name": "GaBiCategories"}}, {"dataSetInternalID": 6, "referenceToFlowDataSet": {"shortDescription": [{"value": "Total use of non renewable primary energy resources (PENRT)", "lang": "en"}, {"value": "Total nicht erneuerbare Primärenergie (PENRT)", "lang": "de"}], "type": "flow data set", "refObjectId": "06159210-646b-4c8d-8583-da9b3b95a6c1", "uri": "../flows/06159210-646b-4c8d-8583-da9b3b95a6c1.xml"}, "exchange direction": "INPUT", "other": {"anies": [{"name": "referenceToUnitGroupDataSet", "value": {"shortDescription": [{"value": "MJ", "lang": "en"}], "type": "unit group data set", "refObjectId": "93a60a57-a3c8-11da-a746-0800200c9a66", "uri": "../unitgroups/93a60a57-a3c8-11da-a746-0800200c9a66.xml"}}, {"value": "34.41", "module": "A1"}, {"value": "11.67", "module": "A2"}, {"value": "54.710039933", "module": "A3"}, {"value": "66.45", "module": "A4"}, {"value": "15.686837", "module": "A5"}, {"value": "0", "module": "B1", "scenario": "S1"}, {"value": "0", "module": "B1", "scenario": "S2"}, {"value": "0", "module": "B1", "scenario": "S3"}, {"value": "0", "module": "B2"}, {"value": "0", "module": "B3"}, {"value": "0", "module": "B4"}, {"value": "0", "module": "B5"}, {"value": "0", "module": "B6"}, {"value": "0", "module": "B7"}, {"value": "0.2169", "module": "C1"}, {"value": "1.934", "module": "C2"}, {"value": "0.001129", "module": "C3"}, {"value": "2.682", "module": "C4"}, {"value": "0.0365008848", "module": "D"}]}, "resolvedFlowVersion": "38.00.000", "flowProperties": [], "typeOfFlow": "Other flow", "classification": {"classHierarchy": "Quantities / Environmental quantities / EPD EN 15804 / LCI indicators", "name": "GaBiCategories"}}, {"dataSetInternalID": 7, "referenceToFlowDataSet": {"shortDescription": [{"value": "Use of secondary material (SM)", "lang": "en"}, {"value": "Einsatz von Sekundärstoffen (SM)", "lang": "de"}], "type": "flow data set", "refObjectId": "c6a1f35f-2d09-4f54-8dfb-97e502e1ce92", "uri": "../flows/c6a1f35f-2d09-4f54-8dfb-97e502e1ce92.xml"}, "exchange direction": "INPUT", "other": {"anies": [{"name": "referenceToUnitGroupDataSet", "value": {"shortDescription": [{"value": "kg", "lang": "en"}], "type": "unit group data set", "refObjectId": "ad38d542-3fe9-439d-9b95-2f5f7752acaf", "uri": "../unitgroups/ad38d542-3fe9-439d-9b95-2f5f7752acaf.xml"}}, {"value": "0.54", "module": "A1"}, {"value": "0", "module": "A2"}, {"value": "0", "module": "A3"}, {"value": "0", "module": "A4"}, {"value": "0", "module": "A5"}, {"value": "0", "module": "B1", "scenario": "S1"}, {"value": "0", "module": "B1", "scenario": "S2"}, {"value": "0", "module": "B1", "scenario": "S3"}, {"value": "0", "module": "B2"}, {"value": "0", "module": "B3"}, {"value": "0", "module": "B4"}, {"value": "0", "module": "B5"}, {"value": "0", "module": "B6"}, {"value": "0", "module": "B7"}, {"value": "0", "module": "C1"}, {"value": "0", "module": "C2"}, {"value": "0", "module": "C3"}, {"value": "0", "module": "C4"}, {"value": "1.37023853294", "module": "D"}]}, "resolvedFlowVersion": "38.00.000", "flowProperties": [], "typeOfFlow": "Other flow", "classification": {"classHierarchy": "Quantities / Environmental quantities / EPD EN 15804 / LCI indicators", "name": "GaBiCategories"}}, {"dataSetInternalID": 8, "referenceToFlowDataSet": {"shortDescription": [{"value": "Use of renewable secondary fuels (RSF)", "lang": "en"}, {"value": "Erneuerbare Sekundärbrennstoffe (RSF)", "lang": "de"}], "type": "flow data set", "refObjectId": "64333088-a55f-4aa2-9a31-c10b07816787", "uri": "../flows/64333088-a55f-4aa2-9a31-c10b07816787.xml"}, "exchange direction": "INPUT", "other": {"anies": [{"name": "referenceToUnitGroupDataSet", "value": {"shortDescription": [{"value": "MJ", "lang": "en"}], "type": "unit group data set", "refObjectId": "93a60a57-a3c8-11da-a746-0800200c9a66", "uri": "../unitgroups/93a60a57-a3c8-11da-a746-0800200c9a66.xml"}}, {"value": "0", "module": "A1"}, {"value": "0", "module": "A2"}, {"value": "0", "module": "A3"}, {"value": "0", "module": "A4"}, {"value": "0", "module": "A5"}, {"value": "0", "module": "B1", "scenario": "S1"}, {"value": "0", "module": "B1", "scenario": "S2"}, {"value": "0", "module": "B1", "scenario": "S3"}, {"value": "0", "module": "B2"}, {"value": "0", "module": "B3"}, {"value": "0", "module": "B4"}, {"value": "0", "module": "B5"}, {"value": "0", "module": "B6"}, {"value": "0", "module": "B7"}, {"value": "0", "module": "C1"}, {"value": "0", "module": "C2"}, {"value": "0", "module": "C3"}, {"value": "0", "module": "C4"}, {"value": "0", "module": "D"}]}, "resolvedFlowVersion": "38.00.000", "flowProperties": [], "typeOfFlow": "Other flow", "classification": {"classHierarchy": "Quantities / Environmental quantities / EPD EN 15804 / LCI indicators", "name": "GaBiCategories"}}, {"dataSetInternalID": 9, "referenceToFlowDataSet": {"shortDescription": [{"value": "Use of non renewable secondary fuels (NRSF)", "lang": "en"}, {"value": "Nicht erneuerbare Sekundärbrennstoffe (NRSF)", "lang": "de"}], "type": "flow data set", "refObjectId": "89def144-d39a-4287-b86f-efde453ddcb2", "uri": "../flows/89def144-d39a-4287-b86f-efde453ddcb2.xml"}, "exchange direction": "INPUT", "other": {"anies": [{"name": "referenceToUnitGroupDataSet", "value": {"shortDescription": [{"value": "MJ", "lang": "en"}], "type": "unit group data set", "refObjectId": "93a60a57-a3c8-11da-a746-0800200c9a66", "uri": "../unitgroups/93a60a57-a3c8-11da-a746-0800200c9a66.xml"}}, {"value": "0", "module": "A1"}, {"value": "0", "module": "A2"}, {"value": "0", "module": "A3"}, {"value": "0", "module": "A4"}, {"value": "0", "module": "A5"}, {"value": "0", "module": "B1", "scenario": "S1"}, {"value": "0", "module": "B1", "scenario": "S2"}, {"value": "0", "module": "B1", "scenario": "S3"}, {"value": "0", "module": "B2"}, {"value": "0", "module": "B3"}, {"value": "0", "module": "B4"}, {"value": "0", "module": "B5"}, {"value": "0", "module": "B6"}, {"value": "0", "module": "B7"}, {"value": "0", "module": "C1"}, {"value": "0", "module": "C2"}, {"value": "0", "module": "C3"}, {"value": "0", "module": "C4"}, {"value": "0", "module": "D"}]}, "resolvedFlowVersion": "38.00.000", "flowProperties": [], "typeOfFlow": "Other flow", "classification": {"classHierarchy": "Quantities / Environmental quantities / EPD EN 15804 / LCI indicators", "name": "GaBiCategories"}}, {"dataSetInternalID": 10, "referenceToFlowDataSet": {"shortDescription": [{"value": "Use of net fresh water (FW)", "lang": "en"}, {"value": "Einsatz von Süßwasserressourcen (FW)", "lang": "de"}], "type": "flow data set", "refObjectId": "3cf952c8-f3a4-461d-8c96-96456ca62246", "uri": "../flows/3cf952c8-f3a4-461d-8c96-96456ca62246.xml"}, "exchange direction": "INPUT", "other": {"anies": [{"name": "referenceToUnitGroupDataSet", "value": {"shortDescription": [{"value": "m^3", "lang": "en"}], "type": "unit group data set", "refObjectId": "cd950537-0a98-4044-9ba7-9f9a68d0a504", "uri": "../unitgroups/cd950537-0a98-4044-9ba7-9f9a68d0a504.xml"}}, {"value": "0.03148", "module": "A1"}, {"value": "0.0007699", "module": "A2"}, {"value": "0.01498", "module": "A3"}, {"value": "0.003329", "module": "A4"}, {"value": "0.009267", "module": "A5"}, {"value": "0", "module": "B1", "scenario": "S1"}, {"value": "0", "module": "B1", "scenario": "S2"}, {"value": "0", "module": "B1", "scenario": "S3"}, {"value": "0", "module": "B2"}, {"value": "0", "module": "B3"}, {"value": "0", "module": "B4"}, {"value": "0", "module": "B5"}, {"value": "0", "module": "B6"}, {"value": "0", "module": "B7"}, {"value": "0.0001334", "module": "C1"}, {"value": "0.0001388", "module": "C2"}, {"value": "2.478E-07", "module": "C3"}, {"value": "0.002538", "module": "C4"}, {"value": "-0.0009885", "module": "D"}]}, "resolvedFlowVersion": "38.00.000", "flowProperties": [], "typeOfFlow": "Other flow", "classification": {"classHierarchy": "Quantities / Environmental quantities / EPD EN 15804 / LCI indicators", "name": "GaBiCategories"}}, {"dataSetInternalID": 11, "referenceToFlowDataSet": {"shortDescription": [{"value": "Hazardous waste disposed (HWD)", "lang": "en"}, {"value": "Gefährlicher Abfall zur Deponie (HWD)", "lang": "de"}], "type": "flow data set", "refObjectId": "430f9e0f-59b2-46a0-8e0d-55e0e84948fc", "uri": "../flows/430f9e0f-59b2-46a0-8e0d-55e0e84948fc.xml"}, "exchange direction": "OUTPUT", "other": {"anies": [{"name": "referenceToUnitGroupDataSet", "value": {"shortDescription": [{"value": "kg", "lang": "en"}], "type": "unit group data set", "refObjectId": "ad38d542-3fe9-439d-9b95-2f5f7752acaf", "uri": "../unitgroups/ad38d542-3fe9-439d-9b95-2f5f7752acaf.xml"}}, {"value": "1.846E-05", "module": "A1"}, {"value": "2.91E-05", "module": "A2"}, {"value": "2.934E-05", "module": "A3"}, {"value": "0.0001112", "module": "A4"}, {"value": "1.483E-05", "module": "A5"}, {"value": "0", "module": "B1", "scenario": "S1"}, {"value": "0", "module": "B1", "scenario": "S2"}, {"value": "0", "module": "B1", "scenario": "S3"}, {"value": "0", "module": "B2"}, {"value": "0", "module": "B3"}, {"value": "0", "module": "B4"}, {"value": "0", "module": "B5"}, {"value": "0", "module": "B6"}, {"value": "0", "module": "B7"}, {"value": "1.205E-07", "module": "C1"}, {"value": "5.036E-06", "module": "C2"}, {"value": "1.101E-09", "module": "C3"}, {"value": "3.03E-06", "module": "C4"}, {"value": "-5.458E-06", "module": "D"}]}, "resolvedFlowVersion": "38.00.000", "flowProperties": [], "typeOfFlow": "Other flow", "classification": {"classHierarchy": "Quantities / Environmental quantities / EPD EN 15804 / LCI indicators", "name": "GaBiCategories"}}, {"dataSetInternalID": 12, "referenceToFlowDataSet": {"shortDescription": [{"value": "Non hazardous waste disposed (NHWD)", "lang": "en"}, {"value": "Entsorgter nicht gefährlicher Abfall (NHWD)", "lang": "de"}], "type": "flow data set", "refObjectId": "b29ef66b-e286-4afa-949f-62f1a7b4d7fa", "uri": "../flows/b29ef66b-e286-4afa-949f-62f1a7b4d7fa.xml"}, "exchange direction": "OUTPUT", "other": {"anies": [{"name": "referenceToUnitGroupDataSet", "value": {"shortDescription": [{"value": "kg", "lang": "en"}], "type": "unit group data set", "refObjectId": "ad38d542-3fe9-439d-9b95-2f5f7752acaf", "uri": "../unitgroups/ad38d542-3fe9-439d-9b95-2f5f7752acaf.xml"}}, {"value": "0.3923", "module": "A1"}, {"value": "0.4493", "module": "A2"}, {"value": "0.4564", "module": "A3"}, {"value": "1.489", "module": "A4"}, {"value": "0.8865", "module": "A5"}, {"value": "0", "module": "B1", "scenario": "S1"}, {"value": "0", "module": "B1", "scenario": "S2"}, {"value": "0", "module": "B1", "scenario": "S3"}, {"value": "0", "module": "B2"}, {"value": "0", "module": "B3"}, {"value": "0", "module": "B4"}, {"value": "0", "module": "B5"}, {"value": "0", "module": "B6"}, {"value": "0", "module": "B7"}, {"value": "0.0006391", "module": "C1"}, {"value": "0.09193", "module": "C2"}, {"value": "3.743E-06", "module": "C3"}, {"value": "14.82", "module": "C4"}, {"value": "-0.01426", "module": "D"}]}, "resolvedFlowVersion": "38.00.000", "flowProperties": [], "typeOfFlow": "Other flow", "classification": {"classHierarchy": "Quantities / Environmental quantities / EPD EN 15804 / LCI indicators", "name": "GaBiCategories"}}, {"dataSetInternalID": 13, "referenceToFlowDataSet": {"shortDescription": [{"value": "Radioactive waste disposed (RWD)", "lang": "en"}, {"value": "Entsorgter radioaktiver Abfall (RWD)", "lang": "de"}], "type": "flow data set", "refObjectId": "3449546e-52ad-4b39-b809-9fb77cea8ff6", "uri": "../flows/3449546e-52ad-4b39-b809-9fb77cea8ff6.xml"}, "exchange direction": "OUTPUT", "other": {"anies": [{"name": "referenceToUnitGroupDataSet", "value": {"shortDescription": [{"value": "kg", "lang": "en"}], "type": "unit group data set", "refObjectId": "ad38d542-3fe9-439d-9b95-2f5f7752acaf", "uri": "../unitgroups/ad38d542-3fe9-439d-9b95-2f5f7752acaf.xml"}}, {"value": "9.295E-05", "module": "A1"}, {"value": "7.509E-05", "module": "A2"}, {"value": "5.203E-05", "module": "A3"}, {"value": "0.0004568", "module": "A4"}, {"value": "4.79E-05", "module": "A5"}, {"value": "0", "module": "B1", "scenario": "S1"}, {"value": "0", "module": "B1", "scenario": "S2"}, {"value": "0", "module": "B1", "scenario": "S3"}, {"value": "0", "module": "B2"}, {"value": "0", "module": "B3"}, {"value": "0", "module": "B4"}, {"value": "0", "module": "B5"}, {"value": "0", "module": "B6"}, {"value": "0", "module": "B7"}, {"value": "1.284E-06", "module": "C1"}, {"value": "1.31E-05", "module": "C2"}, {"value": "3.383E-09", "module": "C3"}, {"value": "1.616E-05", "module": "C4"}, {"value": "-7.421E-06", "module": "D"}]}, "resolvedFlowVersion": "38.00.000", "flowProperties": [], "typeOfFlow": "Other flow", "classification": {"classHierarchy": "Quantities / Environmental quantities / EPD EN 15804 / LCI indicators", "name": "GaBiCategories"}}, {"dataSetInternalID": 14, "referenceToFlowDataSet": {"shortDescription": [{"value": "Components for re-use (CRU)", "lang": "en"}, {"value": "Komponenten für die Wiederverwendung (CRU)", "lang": "de"}], "type": "flow data set", "refObjectId": "a2b32f97-3fc7-4af2-b209-525bc6426f33", "uri": "../flows/a2b32f97-3fc7-4af2-b209-525bc6426f33.xml"}, "exchange direction": "OUTPUT", "other": {"anies": [{"name": "referenceToUnitGroupDataSet", "value": {"shortDescription": [{"value": "kg", "lang": "en"}], "type": "unit group data set", "refObjectId": "ad38d542-3fe9-439d-9b95-2f5f7752acaf", "uri": "../unitgroups/ad38d542-3fe9-439d-9b95-2f5f7752acaf.xml"}}, {"value": "0", "module": "A1"}, {"value": "0", "module": "A2"}, {"value": "0", "module": "A3"}, {"value": "0", "module": "A4"}, {"value": "0", "module": "A5"}, {"value": "0", "module": "B1", "scenario": "S1"}, {"value": "0", "module": "B1", "scenario": "S2"}, {"value": "0", "module": "B1", "scenario": "S3"}, {"value": "0", "module": "B2"}, {"value": "0", "module": "B3"}, {"value": "0", "module": "B4"}, {"value": "0", "module": "B5"}, {"value": "0", "module": "B6"}, {"value": "0", "module": "B7"}, {"value": "0", "module": "C1"}, {"value": "0", "module": "C2"}, {"value": "0", "module": "C3"}, {"value": "0", "module": "C4"}, {"value": "0", "module": "D"}]}, "resolvedFlowVersion": "38.00.000", "flowProperties": [], "typeOfFlow": "Other flow", "classification": {"classHierarchy": "Quantities / Environmental quantities / EPD EN 15804 / LCI indicators", "name": "GaBiCategories"}}, {"dataSetInternalID": 15, "referenceToFlowDataSet": {"shortDescription": [{"value": "Materials for recycling (MFR)", "lang": "en"}, {"value": "Stoffe zum Recycling (MFR)", "lang": "de"}], "type": "flow data set", "refObjectId": "d7fe48a5-4103-49c8-9aae-b0b5dfdbd6ae", "uri": "../flows/d7fe48a5-4103-49c8-9aae-b0b5dfdbd6ae.xml"}, "exchange direction": "OUTPUT", "other": {"anies": [{"name": "referenceToUnitGroupDataSet", "value": {"shortDescription": [{"value": "kg", "lang": "en"}], "type": "unit group data set", "refObjectId": "ad38d542-3fe9-439d-9b95-2f5f7752acaf", "uri": "../unitgroups/ad38d542-3fe9-439d-9b95-2f5f7752acaf.xml"}}, {"value": "0", "module": "A1"}, {"value": "0", "module": "A2"}, {"value": "1.7109030028", "module": "A3"}, {"value": "0", "module": "A4"}, {"value": "0.22633553014", "module": "A5"}, {"value": "0", "module": "B1", "scenario": "S1"}, {"value": "0", "module": "B1", "scenario": "S2"}, {"value": "0", "module": "B1", "scenario": "S3"}, {"value": "0", "module": "B2"}, {"value": "0", "module": "B3"}, {"value": "0", "module": "B4"}, {"value": "0", "module": "B5"}, {"value": "0", "module": "B6"}, {"value": "0", "module": "B7"}, {"value": "0", "module": "C1"}, {"value": "0", "module": "C2"}, {"value": "0", "module": "C3"}, {"value": "0", "module": "C4"}, {"value": "-1.93723853294", "module": "D"}]}, "resolvedFlowVersion": "38.00.000", "flowProperties": [], "typeOfFlow": "Other flow", "classification": {"classHierarchy": "Quantities / Environmental quantities / EPD EN 15804 / LCI indicators", "name": "GaBiCategories"}}, {"dataSetInternalID": 16, "referenceToFlowDataSet": {"shortDescription": [{"value": "Materials for energy recovery (MER)", "lang": "en"}, {"value": "Stoffe für die Energierückgewinnung (MER)", "lang": "de"}], "type": "flow data set", "refObjectId": "59a9181c-3aaf-46ee-8b13-2b3723b6e447", "uri": "../flows/59a9181c-3aaf-46ee-8b13-2b3723b6e447.xml"}, "exchange direction": "OUTPUT", "other": {"anies": [{"name": "referenceToUnitGroupDataSet", "value": {"shortDescription": [{"value": "kg", "lang": "en"}], "type": "unit group data set", "refObjectId": "ad38d542-3fe9-439d-9b95-2f5f7752acaf", "uri": "../unitgroups/ad38d542-3fe9-439d-9b95-2f5f7752acaf.xml"}}, {"value": "0", "module": "A1"}, {"value": "0", "module": "A2"}, {"value": "0", "module": "A3"}, {"value": "0", "module": "A4"}, {"value": "0", "module": "A5"}, {"value": "0", "module": "B1", "scenario": "S1"}, {"value": "0", "module": "B1", "scenario": "S2"}, {"value": "0", "module": "B1", "scenario": "S3"}, {"value": "0", "module": "B2"}, {"value": "0", "module": "B3"}, {"value": "0", "module": "B4"}, {"value": "0", "module": "B5"}, {"value": "0", "module": "B6"}, {"value": "0", "module": "B7"}, {"value": "0", "module": "C1"}, {"value": "0", "module": "C2"}, {"value": "0", "module": "C3"}, {"value": "0", "module": "C4"}, {"value": "0", "module": "D"}]}, "resolvedFlowVersion": "38.00.000", "flowProperties": [], "typeOfFlow": "Other flow", "classification": {"classHierarchy": "Quantities / Environmental quantities / EPD EN 15804 / LCI indicators", "name": "GaBiCategories"}}, {"dataSetInternalID": 17, "referenceToFlowDataSet": {"shortDescription": [{"value": "Exported electrical energy (EEE)", "lang": "en"}, {"value": "Exportierte elektrische Energie (EEE)", "lang": "de"}], "type": "flow data set", "refObjectId": "4da0c987-2b76-40d6-9e9e-82a017aaaf29", "uri": "../flows/4da0c987-2b76-40d6-9e9e-82a017aaaf29.xml"}, "exchange direction": "OUTPUT", "other": {"anies": [{"name": "referenceToUnitGroupDataSet", "value": {"shortDescription": [{"value": "MJ", "lang": "en"}], "type": "unit group data set", "refObjectId": "93a60a57-a3c8-11da-a746-0800200c9a66", "uri": "../unitgroups/93a60a57-a3c8-11da-a746-0800200c9a66.xml"}}, {"value": "0", "module": "A1"}, {"value": "0", "module": "A2"}, {"value": "0.027138689634304", "module": "A3"}, {"value": "0", "module": "A4"}, {"value": "0.392031301165226", "module": "A5"}, {"value": "0", "module": "B1", "scenario": "S1"}, {"value": "0", "module": "B1", "scenario": "S2"}, {"value": "0", "module": "B1", "scenario": "S3"}, {"value": "0", "module": "B2"}, {"value": "0", "module": "B3"}, {"value": "0", "module": "B4"}, {"value": "0", "module": "B5"}, {"value": "0", "module": "B6"}, {"value": "0", "module": "B7"}, {"value": "0", "module": "C1"}, {"value": "0", "module": "C2"}, {"value": "0", "module": "C3"}, {"value": "0", "module": "C4"}, {"value": "-0.41916999079953", "module": "D"}]}, "resolvedFlowVersion": "38.00.000", "flowProperties": [], "typeOfFlow": "Other flow", "classification": {"classHierarchy": "Quantities / Environmental quantities / EPD EN 15804 / LCI indicators", "name": "GaBiCategories"}}, {"dataSetInternalID": 18, "referenceToFlowDataSet": {"shortDescription": [{"value": "Exported thermal energy (EET)", "lang": "en"}, {"value": "Exportierte thermische Energie (EET)", "lang": "de"}], "type": "flow data set", "refObjectId": "98daf38a-7a79-46d3-9a37-2b7bd0955810", "uri": "../flows/98daf38a-7a79-46d3-9a37-2b7bd0955810.xml"}, "exchange direction": "OUTPUT", "other": {"anies": [{"name": "referenceToUnitGroupDataSet", "value": {"shortDescription": [{"value": "MJ", "lang": "en"}], "type": "unit group data set", "refObjectId": "93a60a57-a3c8-11da-a746-0800200c9a66", "uri": "../unitgroups/93a60a57-a3c8-11da-a746-0800200c9a66.xml"}}, {"value": "0", "module": "A1"}, {"value": "0", "module": "A2"}, {"value": "0", "module": "A3"}, {"value": "0", "module": "A4"}, {"value": "0", "module": "A5"}, {"value": "0", "module": "B1", "scenario": "S1"}, {"value": "0", "module": "B1", "scenario": "S2"}, {"value": "0", "module": "B1", "scenario": "S3"}, {"value": "0", "module": "B2"}, {"value": "0", "module": "B3"}, {"value": "0", "module": "B4"}, {"value": "0", "module": "B5"}, {"value": "0", "module": "B6"}, {"value": "0", "module": "B7"}, {"value": "0", "module": "C1"}, {"value": "0", "module": "C2"}, {"value": "0", "module": "C3"}, {"value": "0", "module": "C4"}, {"value": "0", "module": "D"}]}, "resolvedFlowVersion": "38.00.000", "flowProperties": [], "typeOfFlow": "Other flow", "classification": {"classHierarchy": "Quantities / Environmental quantities / EPD EN 15804 / LCI indicators", "name": "GaBiCategories"}}]}, "LCIAResults": {"LCIAResult": [{"referenceToLCIAMethodDataSet": {"shortDescription": [{"value": "Global Warming Potential total (GWP-total)", "lang": "en"}, {"value": "Globales Erwärmungspotenzial total (GWP-total)", "lang": "de"}], "type": "LCIA method data set", "refObjectId": "6a37f984-a4b3-458a-a20a-64418c145fa2", "uri": "../lciamethods/6a37f984-a4b3-458a-a20a-64418c145fa2.xml"}, "other": {"anies": [{"name": "referenceToUnitGroupDataSet", "value": {"shortDescription": [{"value": "kg CO_(2)-Äq.", "lang": "en"}], "type": "unit group data set", "refObjectId": "1ebf3012-d0db-4de2-aefd-ef30cedb0be1", "uri": "../unitgroups/1ebf3012-d0db-4de2-aefd-ef30cedb0be1.xml"}}, {"value": "3.60207425753968", "module": "A1"}, {"value": "0.7936282", "module": "A2"}, {"value": "3.1840704922161", "module": "A3"}, {"value": "4.847282", "module": "A4"}, {"value": "1.67152951587302", "module": "A5"}, {"value": "-1.768", "module": "B1", "scenario": "S1"}, {"value": "-0.943", "module": "B1", "scenario": "S2"}, {"value": "0", "module": "B1", "scenario": "S3"}, {"value": "0", "module": "B2"}, {"value": "0", "module": "B3"}, {"value": "0", "module": "B4"}, {"value": "0", "module": "B5"}, {"value": "0", "module": "B6"}, {"value": "0", "module": "B7"}, {"value": "0.00887398", "module": "C1"}, {"value": "0.1274965", "module": "C2"}, {"value": "6.289783E-05", "module": "C3"}, {"value": "1.7255691743712", "module": "C4"}, {"value": "-0.1375964", "module": "D"}]}}, {"referenceToLCIAMethodDataSet": {"shortDescription": [{"value": "Global Warming Potential fossil fuels (GWP-fossil)", "lang": "en"}, {"value": "Globales Erwärmungspotenzial fossil (GWP-fossil)", "lang": "de"}], "type": "LCIA method data set", "refObjectId": "5f635281-343e-44fb-83df-1971b155e6b6", "uri": "../lciamethods/5f635281-343e-44fb-83df-1971b155e6b6.xml"}, "other": {"anies": [{"name": "referenceToUnitGroupDataSet", "value": {"shortDescription": [{"value": "kg CO_(2)-Äq.", "lang": "en"}], "type": "unit group data set", "refObjectId": "1ebf3012-d0db-4de2-aefd-ef30cedb0be1", "uri": "../unitgroups/1ebf3012-d0db-4de2-aefd-ef30cedb0be1.xml"}}, {"value": "5.398", "module": "A1"}, {"value": "0.7928", "module": "A2"}, {"value": "3.67", "module": "A3"}, {"value": "4.843", "module": "A4"}, {"value": "0.9641", "module": "A5"}, {"value": "0", "module": "B1", "scenario": "S1"}, {"value": "0", "module": "B1", "scenario": "S2"}, {"value": "0", "module": "B1", "scenario": "S3"}, {"value": "0", "module": "B2"}, {"value": "0", "module": "B3"}, {"value": "0", "module": "B4"}, {"value": "0", "module": "B5"}, {"value": "0", "module": "B6"}, {"value": "0", "module": "B7"}, {"value": "0.008792", "module": "C1"}, {"value": "0.1274", "module": "C2"}, {"value": "6.18E-05", "module": "C3"}, {"value": "0.1003", "module": "C4"}, {"value": "-0.1372", "module": "D"}]}}, {"referenceToLCIAMethodDataSet": {"shortDescription": [{"value": "Global Warming Potential biogenic (GWP-biogenic)", "lang": "en"}, {"value": "Globales Erwärmungspotenzial biogen (GWP-biogenic)", "lang": "de"}], "type": "LCIA method data set", "refObjectId": "2356e1ab-0185-4db5-86e5-16de51c7485c", "uri": "../lciamethods/2356e1ab-0185-4db5-86e5-16de51c7485c.xml"}, "other": {"anies": [{"name": "referenceToUnitGroupDataSet", "value": {"shortDescription": [{"value": "kg CO_(2)-Äq.", "lang": "en"}], "type": "unit group data set", "refObjectId": "1ebf3012-d0db-4de2-aefd-ef30cedb0be1", "uri": "../unitgroups/1ebf3012-d0db-4de2-aefd-ef30cedb0be1.xml"}}, {"value": "-1.79829474246032", "module": "A1"}, {"value": "0.0003519", "module": "A2"}, {"value": "-0.493288507783901", "module": "A3"}, {"value": "0.001595", "module": "A4"}, {"value": "0.706643015873016", "module": "A5"}, {"value": "0", "module": "B1", "scenario": "S1"}, {"value": "0", "module": "B1", "scenario": "S2"}, {"value": "0", "module": "B1", "scenario": "S3"}, {"value": "0", "module": "B2"}, {"value": "0", "module": "B3"}, {"value": "0", "module": "B4"}, {"value": "0", "module": "B5"}, {"value": "0", "module": "B6"}, {"value": "0", "module": "B7"}, {"value": "6.153E-05", "module": "C1"}, {"value": "5.196E-05", "module": "C2"}, {"value": "1.024E-06", "module": "C3"}, {"value": "1.6252179343712", "module": "C4"}, {"value": "-0.000152", "module": "D"}]}}, {"referenceToLCIAMethodDataSet": {"shortDescription": [{"value": "Global Warming Potential luluc (GWP-luluc)", "lang": "en"}, {"value": "Globales Erwärmungspotenzial luluc (GWP-luluc)", "lang": "de"}], "type": "LCIA method data set", "refObjectId": "4331bbdb-978a-490d-8707-eeb047f01a55", "uri": "../lciamethods/4331bbdb-978a-490d-8707-eeb047f01a55.xml"}, "other": {"anies": [{"name": "referenceToUnitGroupDataSet", "value": {"shortDescription": [{"value": "kg CO_(2)-Äq.", "lang": "en"}], "type": "unit group data set", "refObjectId": "1ebf3012-d0db-4de2-aefd-ef30cedb0be1", "uri": "../unitgroups/1ebf3012-d0db-4de2-aefd-ef30cedb0be1.xml"}}, {"value": "0.002369", "module": "A1"}, {"value": "0.0004763", "module": "A2"}, {"value": "0.007359", "module": "A3"}, {"value": "0.002687", "module": "A4"}, {"value": "0.0007865", "module": "A5"}, {"value": "0", "module": "B1", "scenario": "S1"}, {"value": "0", "module": "B1", "scenario": "S2"}, {"value": "0", "module": "B1", "scenario": "S3"}, {"value": "0", "module": "B2"}, {"value": "0", "module": "B3"}, {"value": "0", "module": "B4"}, {"value": "0", "module": "B5"}, {"value": "0", "module": "B6"}, {"value": "0", "module": "B7"}, {"value": "2.045E-05", "module": "C1"}, {"value": "4.454E-05", "module": "C2"}, {"value": "7.383E-08", "module": "C3"}, {"value": "5.124E-05", "module": "C4"}, {"value": "-0.0002444", "module": "D"}]}}, {"referenceToLCIAMethodDataSet": {"shortDescription": [{"value": "Depletion potential of the stratospheric ozone layer (ODP)", "lang": "en"}, {"value": "Abbau Potential der stratosphärischen Ozonschicht (ODP)", "lang": "de"}], "type": "LCIA method data set", "refObjectId": "b5c629d6-def3-11e6-bf01-fe55135034f3", "uri": "../lciamethods/b5c629d6-def3-11e6-bf01-fe55135034f3.xml"}, "other": {"anies": [{"name": "referenceToUnitGroupDataSet", "value": {"shortDescription": [{"value": "kg CFC11-Äq.", "lang": "en"}], "type": "unit group data set", "refObjectId": "d9e957c9-7309-4474-bf3a-7777df6c4e5b", "uri": "../unitgroups/d9e957c9-7309-4474-bf3a-7777df6c4e5b.xml"}}, {"value": "2.446E-07", "module": "A1"}, {"value": "1.677E-07", "module": "A2"}, {"value": "2.108E-07", "module": "A3"}, {"value": "1.022E-06", "module": "A4"}, {"value": "9.821E-08", "module": "A5"}, {"value": "0", "module": "B1", "scenario": "S1"}, {"value": "0", "module": "B1", "scenario": "S2"}, {"value": "0", "module": "B1", "scenario": "S3"}, {"value": "0", "module": "B2"}, {"value": "0", "module": "B3"}, {"value": "0", "module": "B4"}, {"value": "0", "module": "B5"}, {"value": "0", "module": "B6"}, {"value": "0", "module": "B7"}, {"value": "7.404E-10", "module": "C1"}, {"value": "2.895E-08", "module": "C2"}, {"value": "2.503E-12", "module": "C3"}, {"value": "3.322E-08", "module": "C4"}, {"value": "-1.373E-08", "module": "D"}]}}, {"referenceToLCIAMethodDataSet": {"shortDescription": [{"value": "Acidification potential of land and water (AP)", "lang": "en"}, {"value": "Versauerungspotenzial von Boden und Wasser (AP)", "lang": "de"}], "type": "LCIA method data set", "refObjectId": "b5c611c6-def3-11e6-bf01-fe55135034f3", "uri": "../lciamethods/b5c611c6-def3-11e6-bf01-fe55135034f3.xml"}, "other": {"anies": [{"name": "referenceToUnitGroupDataSet", "value": {"shortDescription": [{"value": "mol H^(+)-Äq.", "lang": "en"}], "type": "unit group data set", "refObjectId": "42e089ac-92bf-4bf2-8ca1-5fc40d18f2ed", "uri": "../unitgroups/42e089ac-92bf-4bf2-8ca1-5fc40d18f2ed.xml"}}, {"value": "0.01876", "module": "A1"}, {"value": "0.006895", "module": "A2"}, {"value": "0.01736", "module": "A3"}, {"value": "0.1021", "module": "A4"}, {"value": "0.007246", "module": "A5"}, {"value": "0", "module": "B1", "scenario": "S1"}, {"value": "0", "module": "B1", "scenario": "S2"}, {"value": "0", "module": "B1", "scenario": "S3"}, {"value": "0", "module": "B2"}, {"value": "0", "module": "B3"}, {"value": "0", "module": "B4"}, {"value": "0", "module": "B5"}, {"value": "0", "module": "B6"}, {"value": "0", "module": "B7"}, {"value": "5.131E-05", "module": "C1"}, {"value": "0.0005207", "module": "C2"}, {"value": "1.846E-07", "module": "C3"}, {"value": "0.0007641", "module": "C4"}, {"value": "-0.0005674", "module": "D"}]}}, {"referenceToLCIAMethodDataSet": {"shortDescription": [{"value": "Eutrophication potential aquatic freshwater (EP-freshwater)", "lang": "en"}, {"value": "Eutrophierungspotenzial Süßwasser (EP-freshwater)", "lang": "de"}], "type": "LCIA method data set", "refObjectId": "b53ec18f-7377-4ad3-86eb-cc3f4f276b2b", "uri": "../lciamethods/b53ec18f-7377-4ad3-86eb-cc3f4f276b2b.xml"}, "other": {"anies": [{"name": "referenceToUnitGroupDataSet", "value": {"shortDescription": [{"value": "kg PO_(4)-Äq.", "lang": "en"}], "type": "unit group data set", "refObjectId": "0429039d-a61d-4590-ba67-aa4a20a810a1", "uri": "../unitgroups/0429039d-a61d-4590-ba67-aa4a20a810a1.xml"}}, {"value": "9.141E-05", "module": "A1"}, {"value": "7.408E-06", "module": "A2"}, {"value": "0.0004613", "module": "A3"}, {"value": "2.761E-05", "module": "A4"}, {"value": "3.889E-05", "module": "A5"}, {"value": "0", "module": "B1", "scenario": "S1"}, {"value": "0", "module": "B1", "scenario": "S2"}, {"value": "0", "module": "B1", "scenario": "S3"}, {"value": "0", "module": "B2"}, {"value": "0", "module": "B3"}, {"value": "0", "module": "B4"}, {"value": "0", "module": "B5"}, {"value": "0", "module": "B6"}, {"value": "0", "module": "B7"}, {"value": "9.388E-07", "module": "C1"}, {"value": "1.001E-06", "module": "C2"}, {"value": "9.242E-09", "module": "C3"}, {"value": "5.301E-06", "module": "C4"}, {"value": "-7.147E-06", "module": "D"}]}}, {"referenceToLCIAMethodDataSet": {"shortDescription": [{"value": "Eutrophication potential aquatic marine (EP-marine)", "lang": "en"}, {"value": "Eutrophierungspotenzial Salzwasser (EP-marine)", "lang": "de"}], "type": "LCIA method data set", "refObjectId": "b5c619fa-def3-11e6-bf01-fe55135034f3", "uri": "../lciamethods/b5c619fa-def3-11e6-bf01-fe55135034f3.xml"}, "other": {"anies": [{"name": "referenceToUnitGroupDataSet", "value": {"shortDescription": [{"value": "kg N-Äq.", "lang": "en"}], "type": "unit group data set", "refObjectId": "d05bb823-ecdf-4686-8c40-bf1d9257859f", "uri": "../unitgroups/d05bb823-ecdf-4686-8c40-bf1d9257859f.xml"}}, {"value": "0.004505", "module": "A1"}, {"value": "0.002484", "module": "A2"}, {"value": "0.003657", "module": "A3"}, {"value": "0.02562", "module": "A4"}, {"value": "0.001591", "module": "A5"}, {"value": "0", "module": "B1", "scenario": "S1"}, {"value": "0", "module": "B1", "scenario": "S2"}, {"value": "0", "module": "B1", "scenario": "S3"}, {"value": "0", "module": "B2"}, {"value": "0", "module": "B3"}, {"value": "0", "module": "B4"}, {"value": "0", "module": "B5"}, {"value": "0", "module": "B6"}, {"value": "0", "module": "B7"}, {"value": "6.511E-06", "module": "C1"}, {"value": "0.0001545", "module": "C2"}, {"value": "2.974E-08", "module": "C3"}, {"value": "0.0002692", "module": "C4"}, {"value": "-0.0001205", "module": "D"}]}}, {"referenceToLCIAMethodDataSet": {"shortDescription": [{"value": "Eutrophication potential terrestrial (EP-terrestrial)", "lang": "en"}, {"value": "Eutrophierungspotenzial Land (EP-terrestrial)", "lang": "de"}], "type": "LCIA method data set", "refObjectId": "b5c614d2-def3-11e6-bf01-fe55135034f3", "uri": "../lciamethods/b5c614d2-def3-11e6-bf01-fe55135034f3.xml"}, "other": {"anies": [{"name": "referenceToUnitGroupDataSet", "value": {"shortDescription": [{"value": "mol N-Äq.", "lang": "en"}], "type": "unit group data set", "refObjectId": "71b4d617-0ec9-4d3f-b65e-e438940c2401", "uri": "../unitgroups/71b4d617-0ec9-4d3f-b65e-e438940c2401.xml"}}, {"value": "0.0518", "module": "A1"}, {"value": "0.02737", "module": "A2"}, {"value": "0.04026", "module": "A3"}, {"value": "0.2847", "module": "A4"}, {"value": "0.01779", "module": "A5"}, {"value": "0", "module": "B1", "scenario": "S1"}, {"value": "0", "module": "B1", "scenario": "S2"}, {"value": "0", "module": "B1", "scenario": "S3"}, {"value": "0", "module": "B2"}, {"value": "0", "module": "B3"}, {"value": "0", "module": "B4"}, {"value": "0", "module": "B5"}, {"value": "0", "module": "B6"}, {"value": "0", "module": "B7"}, {"value": "8.023E-05", "module": "C1"}, {"value": "0.001708", "module": "C2"}, {"value": "4.591E-07", "module": "C3"}, {"value": "0.003033", "module": "C4"}, {"value": "-0.001365", "module": "D"}]}}, {"referenceToLCIAMethodDataSet": {"shortDescription": [{"value": "Formation potential of tropospheric ozone photochemical oxidants (POCP)", "lang": "en"}, {"value": "Bildungspotential für troposphärisches Ozon (POCP)", "lang": "de"}], "type": "LCIA method data set", "refObjectId": "b5c610fe-def3-11e6-bf01-fe55135034f3", "uri": "../lciamethods/b5c610fe-def3-11e6-bf01-fe55135034f3.xml"}, "other": {"anies": [{"name": "referenceToUnitGroupDataSet", "value": {"shortDescription": [{"value": "kg NMVOC-Äq.", "lang": "en"}], "type": "unit group data set", "refObjectId": "d27c25f8-fbc1-44c6-b47b-4adbae4199c6", "uri": "../unitgroups/d27c25f8-fbc1-44c6-b47b-4adbae4199c6.xml"}}, {"value": "0.01337", "module": "A1"}, {"value": "0.007367", "module": "A2"}, {"value": "0.01116", "module": "A3"}, {"value": "0.07496", "module": "A4"}, {"value": "0.005115", "module": "A5"}, {"value": "0", "module": "B1", "scenario": "S1"}, {"value": "0", "module": "B1", "scenario": "S2"}, {"value": "0", "module": "B1", "scenario": "S3"}, {"value": "0", "module": "B2"}, {"value": "0", "module": "B3"}, {"value": "0", "module": "B4"}, {"value": "0", "module": "B5"}, {"value": "0", "module": "B6"}, {"value": "0", "module": "B7"}, {"value": "2.036E-05", "module": "C1"}, {"value": "0.0005231", "module": "C2"}, {"value": "9.125E-08", "module": "C3"}, {"value": "0.0008444", "module": "C4"}, {"value": "-0.0004788", "module": "D"}]}}, {"referenceToLCIAMethodDataSet": {"shortDescription": [{"value": "Abiotic depletion potential for non fossil resources (ADPE)", "lang": "en"}, {"value": "Potenzial für den abiotischen Abbau nicht fossiler Ressourcen (ADPE)", "lang": "de"}], "type": "LCIA method data set", "refObjectId": "b2ad6494-c78d-11e6-9d9d-cec0c932ce01", "uri": "../lciamethods/b2ad6494-c78d-11e6-9d9d-cec0c932ce01.xml"}, "other": {"anies": [{"name": "referenceToUnitGroupDataSet", "value": {"shortDescription": [{"value": "kg Sb-Äq.", "lang": "en"}], "type": "unit group data set", "refObjectId": "54ccd2d9-a32a-4fc2-923d-f2c8c93e89d4", "uri": "../unitgroups/54ccd2d9-a32a-4fc2-923d-f2c8c93e89d4.xml"}}, {"value": "1.131E-05", "module": "A1"}, {"value": "1.288E-06", "module": "A2"}, {"value": "9.763E-07", "module": "A3"}, {"value": "6.091E-06", "module": "A4"}, {"value": "7.026E-06", "module": "A5"}, {"value": "0", "module": "B1", "scenario": "S1"}, {"value": "0", "module": "B1", "scenario": "S2"}, {"value": "0", "module": "B1", "scenario": "S3"}, {"value": "0", "module": "B2"}, {"value": "0", "module": "B3"}, {"value": "0", "module": "B4"}, {"value": "0", "module": "B5"}, {"value": "0", "module": "B6"}, {"value": "0", "module": "B7"}, {"value": "1.198E-08", "module": "C1"}, {"value": "2.482E-07", "module": "C2"}, {"value": "1.037E-10", "module": "C3"}, {"value": "9.952E-08", "module": "C4"}, {"value": "-1.146E-07", "module": "D"}]}}, {"referenceToLCIAMethodDataSet": {"shortDescription": [{"value": "Abiotic depletion potential for fossil resources (ADPF)", "lang": "en"}, {"value": "Potenzial für den abiotischen Abbau fossiler Brennstoffe (ADPF)", "lang": "de"}], "type": "LCIA method data set", "refObjectId": "b2ad6110-c78d-11e6-9d9d-cec0c932ce01", "uri": "../lciamethods/b2ad6110-c78d-11e6-9d9d-cec0c932ce01.xml"}, "other": {"anies": [{"name": "referenceToUnitGroupDataSet", "value": {"shortDescription": [{"value": "MJ", "lang": "en"}], "type": "unit group data set", "refObjectId": "93a60a57-a3c8-11da-a746-0800200c9a66", "uri": "../unitgroups/93a60a57-a3c8-11da-a746-0800200c9a66.xml"}}, {"value": "27.83", "module": "A1"}, {"value": "11.43", "module": "A2"}, {"value": "42.64", "module": "A3"}, {"value": "66.36", "module": "A4"}, {"value": "13.89", "module": "A5"}, {"value": "0", "module": "B1", "scenario": "S1"}, {"value": "0", "module": "B1", "scenario": "S2"}, {"value": "0", "module": "B1", "scenario": "S3"}, {"value": "0", "module": "B2"}, {"value": "0", "module": "B3"}, {"value": "0", "module": "B4"}, {"value": "0", "module": "B5"}, {"value": "0", "module": "B6"}, {"value": "0", "module": "B7"}, {"value": "0.1809", "module": "C1"}, {"value": "1.922", "module": "C2"}, {"value": "0.000838", "module": "C3"}, {"value": "2.549", "module": "C4"}, {"value": "-2.288", "module": "D"}]}}, {"referenceToLCIAMethodDataSet": {"shortDescription": [{"value": "Water use (WDP)", "lang": "en"}, {"value": "Wassernutzung (WDP)", "lang": "de"}], "type": "LCIA method data set", "refObjectId": "b2ad66ce-c78d-11e6-9d9d-cec0c932ce01", "uri": "../lciamethods/b2ad66ce-c78d-11e6-9d9d-cec0c932ce01.xml"}, "other": {"anies": [{"name": "referenceToUnitGroupDataSet", "value": {"shortDescription": [{"value": "m^(3) world-Äq. deprived", "lang": "en"}], "type": "unit group data set", "refObjectId": "6ae2df01-888e-46c8-b17d-49fa3869b476", "uri": "../unitgroups/6ae2df01-888e-46c8-b17d-49fa3869b476.xml"}}, {"value": "1.397", "module": "A1"}, {"value": "0.03852", "module": "A2"}, {"value": "0.8391", "module": "A3"}, {"value": "0.1376", "module": "A4"}, {"value": "0.3729", "module": "A5"}, {"value": "0", "module": "B1", "scenario": "S1"}, {"value": "0", "module": "B1", "scenario": "S2"}, {"value": "0", "module": "B1", "scenario": "S3"}, {"value": "0", "module": "B2"}, {"value": "0", "module": "B3"}, {"value": "0", "module": "B4"}, {"value": "0", "module": "B5"}, {"value": "0", "module": "B6"}, {"value": "0", "module": "B7"}, {"value": "0.002026", "module": "C1"}, {"value": "0.005348", "module": "C2"}, {"value": "3.284E-06", "module": "C3"}, {"value": "0.007996", "module": "C4"}, {"value": "-0.03064", "module": "D"}]}}, {"referenceToLCIAMethodDataSet": {"shortDescription": [{"value": "Incidence of disease due to PM emissions (PM)", "lang": "en"}, {"value": "Auftreten von Krankheiten aufgrund von Feinstaubemissionen (PM)", "lang": "de"}], "type": "LCIA method data set", "refObjectId": "b5c602c6-def3-11e6-bf01-fe55135034f3", "uri": "../lciamethods/b5c602c6-def3-11e6-bf01-fe55135034f3.xml"}, "other": {"anies": [{"name": "referenceToUnitGroupDataSet", "value": {"shortDescription": [{"value": "Disease incidence", "lang": "en"}], "type": "unit group data set", "refObjectId": "3883559b-648f-4afc-8ba2-0bd24f3affa3", "uri": "../unitgroups/3883559b-648f-4afc-8ba2-0bd24f3affa3.xml"}}, {"value": "1.98E-07", "module": "A1"}, {"value": "6.71E-08", "module": "A2"}, {"value": "2.374E-07", "module": "A3"}, {"value": "2.297E-07", "module": "A4"}, {"value": "5.014E-08", "module": "A5"}, {"value": "0", "module": "B1", "scenario": "S1"}, {"value": "0", "module": "B1", "scenario": "S2"}, {"value": "0", "module": "B1", "scenario": "S3"}, {"value": "0", "module": "B2"}, {"value": "0", "module": "B3"}, {"value": "0", "module": "B4"}, {"value": "0", "module": "B5"}, {"value": "0", "module": "B6"}, {"value": "0", "module": "B7"}, {"value": "1.342E-10", "module": "C1"}, {"value": "8.865E-09", "module": "C2"}, {"value": "8.478E-13", "module": "C3"}, {"value": "1.492E-08", "module": "C4"}, {"value": "-6.103E-09", "module": "D"}]}}, {"referenceToLCIAMethodDataSet": {"shortDescription": [{"value": "Human exposure efficiency relative to U235 (IR)", "lang": "en"}, {"value": "Wirkung durch Exposition des Menschen mit U235 (IR)", "lang": "de"}], "type": "LCIA method data set", "refObjectId": "b5c632be-def3-11e6-bf01-fe55135034f3", "uri": "../lciamethods/b5c632be-def3-11e6-bf01-fe55135034f3.xml"}, "other": {"anies": [{"name": "referenceToUnitGroupDataSet", "value": {"shortDescription": [{"value": "kBq U235-Äq.", "lang": "en"}], "type": "unit group data set", "refObjectId": "456b05bf-1415-44a9-9993-02452f554c09", "uri": "../unitgroups/456b05bf-1415-44a9-9993-02452f554c09.xml"}}, {"value": "0.08034", "module": "A1"}, {"value": "0.04773", "module": "A2"}, {"value": "0.03676", "module": "A3"}, {"value": "0.2866", "module": "A4"}, {"value": "0.04027", "module": "A5"}, {"value": "0", "module": "B1", "scenario": "S1"}, {"value": "0", "module": "B1", "scenario": "S2"}, {"value": "0", "module": "B1", "scenario": "S3"}, {"value": "0", "module": "B2"}, {"value": "0", "module": "B3"}, {"value": "0", "module": "B4"}, {"value": "0", "module": "B5"}, {"value": "0", "module": "B6"}, {"value": "0", "module": "B7"}, {"value": "0.001563", "module": "C1"}, {"value": "0.008399", "module": "C2"}, {"value": "2.635E-06", "module": "C3"}, {"value": "0.01054", "module": "C4"}, {"value": "-0.007802", "module": "D"}]}}, {"referenceToLCIAMethodDataSet": {"shortDescription": [{"value": "Comparative toxic unit for ecosystems (ETP-fw)", "lang": "en"}, {"value": "Toxizitätsvergleichseinheit für Ökosysteme (ETP-fw)", "lang": "de"}], "type": "LCIA method data set", "refObjectId": "ee1082d1-b0f7-43ca-a1f0-21e2a4a74511", "uri": "../lciamethods/ee1082d1-b0f7-43ca-a1f0-21e2a4a74511.xml"}, "other": {"anies": [{"name": "referenceToUnitGroupDataSet", "value": {"shortDescription": [{"value": "CTUe", "lang": "en"}], "type": "unit group data set", "refObjectId": "aa959ded-f1eb-4efb-9c5c-2d60be36b3e6", "uri": "../unitgroups/aa959ded-f1eb-4efb-9c5c-2d60be36b3e6.xml"}}, {"value": "85.45", "module": "A1"}, {"value": "9.96", "module": "A2"}, {"value": "20.08", "module": "A3"}, {"value": "47.64", "module": "A4"}, {"value": "17.28", "module": "A5"}, {"value": "0", "module": "B1", "scenario": "S1"}, {"value": "0", "module": "B1", "scenario": "S2"}, {"value": "0", "module": "B1", "scenario": "S3"}, {"value": "0", "module": "B2"}, {"value": "0", "module": "B3"}, {"value": "0", "module": "B4"}, {"value": "0", "module": "B5"}, {"value": "0", "module": "B6"}, {"value": "0", "module": "B7"}, {"value": "0.1239", "module": "C1"}, {"value": "1.538", "module": "C2"}, {"value": "0.0007229", "module": "C3"}, {"value": "1.544", "module": "C4"}, {"value": "-1.899", "module": "D"}]}}, {"referenceToLCIAMethodDataSet": {"shortDescription": [{"value": "Comparative toxic unit for humans (carcinogenic) (HTP-c)", "lang": "en"}, {"value": "Toxizitätsvergleichseinheit für Menschen (krebserregend) (HTP-c)", "lang": "de"}], "type": "LCIA method data set", "refObjectId": "2299222a-bbd8-474f-9d4f-4dd1f18aea7c", "uri": "../lciamethods/2299222a-bbd8-474f-9d4f-4dd1f18aea7c.xml"}, "other": {"anies": [{"name": "referenceToUnitGroupDataSet", "value": {"shortDescription": [{"value": "CTUh", "lang": "en"}], "type": "unit group data set", "refObjectId": "d4c9523e-2d7e-49fd-8469-998f547d3a70", "uri": "../unitgroups/d4c9523e-2d7e-49fd-8469-998f547d3a70.xml"}}, {"value": "2.679E-09", "module": "A1"}, {"value": "4.395E-10", "module": "A2"}, {"value": "1.021E-09", "module": "A3"}, {"value": "2.343E-09", "module": "A4"}, {"value": "3.207E-09", "module": "A5"}, {"value": "0", "module": "B1", "scenario": "S1"}, {"value": "0", "module": "B1", "scenario": "S2"}, {"value": "0", "module": "B1", "scenario": "S3"}, {"value": "0", "module": "B2"}, {"value": "0", "module": "B3"}, {"value": "0", "module": "B4"}, {"value": "0", "module": "B5"}, {"value": "0", "module": "B6"}, {"value": "0", "module": "B7"}, {"value": "3.199E-12", "module": "C1"}, {"value": "4.324E-11", "module": "C2"}, {"value": "2.252E-14", "module": "C3"}, {"value": "3.686E-11", "module": "C4"}, {"value": "-1.793E-10", "module": "D"}]}}, {"referenceToLCIAMethodDataSet": {"shortDescription": [{"value": "Comparative toxic unit for humans (noncarcinogenic) (HTP-nc)", "lang": "en"}, {"value": "Toxizitätsvergleichseinheit für Menschen (nicht krebserregend) (HTP-nc)", "lang": "de"}], "type": "LCIA method data set", "refObjectId": "3af763a5-b7a1-48c9-9cee-1f223481fcef", "uri": "../lciamethods/3af763a5-b7a1-48c9-9cee-1f223481fcef.xml"}, "other": {"anies": [{"name": "referenceToUnitGroupDataSet", "value": {"shortDescription": [{"value": "CTUh", "lang": "en"}], "type": "unit group data set", "refObjectId": "d4c9523e-2d7e-49fd-8469-998f547d3a70", "uri": "../unitgroups/d4c9523e-2d7e-49fd-8469-998f547d3a70.xml"}}, {"value": "6.616E-08", "module": "A1"}, {"value": "1.115E-08", "module": "A2"}, {"value": "2.845E-08", "module": "A3"}, {"value": "4.526E-08", "module": "A4"}, {"value": "1.887E-08", "module": "A5"}, {"value": "0", "module": "B1", "scenario": "S1"}, {"value": "0", "module": "B1", "scenario": "S2"}, {"value": "0", "module": "B1", "scenario": "S3"}, {"value": "0", "module": "B2"}, {"value": "0", "module": "B3"}, {"value": "0", "module": "B4"}, {"value": "0", "module": "B5"}, {"value": "0", "module": "B6"}, {"value": "0", "module": "B7"}, {"value": "1.091E-10", "module": "C1"}, {"value": "1.677E-09", "module": "C2"}, {"value": "6.649E-13", "module": "C3"}, {"value": "9.962E-10", "module": "C4"}, {"value": "-1.829E-09", "module": "D"}]}}, {"referenceToLCIAMethodDataSet": {"shortDescription": [{"value": "Soil quality index (SQP)", "lang": "en"}, {"value": "Bodenqualitätsindex (SQP)", "lang": "de"}], "type": "LCIA method data set", "refObjectId": "b2ad6890-c78d-11e6-9d9d-cec0c932ce01", "uri": "../lciamethods/b2ad6890-c78d-11e6-9d9d-cec0c932ce01.xml"}, "other": {"anies": [{"name": "referenceToUnitGroupDataSet", "value": {"shortDescription": [{"value": "SQP", "lang": "en"}], "type": "unit group data set", "refObjectId": "f130951c-e67f-4f7f-8dd4-665de3974e18", "uri": "../unitgroups/f130951c-e67f-4f7f-8dd4-665de3974e18.xml"}}, {"value": "100.1", "module": "A1"}, {"value": "7.491", "module": "A2"}, {"value": "77.98", "module": "A3"}, {"value": "25.18", "module": "A4"}, {"value": "9.147", "module": "A5"}, {"value": "0", "module": "B1", "scenario": "S1"}, {"value": "0", "module": "B1", "scenario": "S2"}, {"value": "0", "module": "B1", "scenario": "S3"}, {"value": "0", "module": "B2"}, {"value": "0", "module": "B3"}, {"value": "0", "module": "B4"}, {"value": "0", "module": "B5"}, {"value": "0", "module": "B6"}, {"value": "0", "module": "B7"}, {"value": "0.04418", "module": "C1"}, {"value": "1.325", "module": "C2"}, {"value": "0.000626", "module": "C3"}, {"value": "4.848", "module": "C4"}, {"value": "-33.44", "module": "D"}]}}]}, "otherAttributes": {"{http://www.indata.network/EPD/2019}epd-version": "1.2"}, "version": "1.1", "locations": "../ILCDLocations.xml"}