{"processInformation": {"dataSetInformation": {"UUID": "b167f5ee-b627-4801-be85-26e61fb26c3c", "name": {"baseName": [{"value": "KTV Atrium Flex", "lang": "en"}, {"value": "KTV Atrium Flex", "lang": "de"}], "functionalUnitFlowProperties": [{"lang": "en"}]}, "classificationInformation": {"classification": [{"class": [{"value": "Komponenten von Fenstern und Vorhangfassaden", "level": 0, "classId": "7"}, {"value": "Antriebssysteme", "level": 1, "classId": "7.7"}, {"value": "elektrisch", "level": 2, "classId": "7.7.02"}], "name": "OEKOBAU.DAT"}, {"class": [{"value": "02 Building products", "level": 0}, {"value": "Doors, windows, shutters, and related products", "level": 1}, {"value": "Automatic doors, automatic gates, and revolving door systems", "level": 2}], "name": "IBUCategories"}]}, "generalComment": [{"value": "The KTV Atrium Flex door range is a breakthrough in design with technology: The revolving door is driven by an electromagnetic direct drive - the dormakaba FLEX Direct Drive technology complements the design intent of modern architecture. It is unique, elegant and leaves an impression that is lasting and timeless.\n\nFor the use and application of the product the respective national provisions at the place of use apply. For the KTV Atrium Flex the standards which can be applied are the following:\n\n20111765/EU ROHS3 Directive\nISO 13849-1: Safety of machinery - Safety-related parts of control systems - Part 1: General principles for design.\nISO 12100: Safety of machinery - Basic concepts - Risk assessment and risk reduction \nEN 16005: Power operated pedestrian doorsets - Safety in use - Requirements and test methods \nEN 61000 - 6 - 2: Electromagnetic compatibility (EMC). Part 6-2: Generic standards: Interference resistance for industrial environments \nEN 61000 - 6 - 3: Electromagnetic compatibility (EMC). Part 6-3: Generic standards: Emission standard for residential, commercial and light-industrial environments.\nEN 61000 - 3 - 2: Electromagnetic compatibility-3-2: Limits - Limits for harmonic current emissions\nEN 61000 - 3 - 3: Electromagnetic compatibility-3-3: Limits - Limitation of voltage changes, voltage fluctuations and flicker in public low-voltage supply systems\nEN 55022: Information technology equipment - Radio disturbance characteristics - Limits and methods of measurement\nEN 60335 - 1: Safety of household and similar electrical appliances. Part 1: General requirements\nEN 60335-2-103: Household and similar electrical appliances. Safety-Particular requirements for drives for gates, doors and windows\nDIN 18650-1: Powered pedestrian doors.\nPart 1: Product requirements and test\nmethods\nDIN 18650-2: Powered pedestrian doors.\nPart 2: Safety at powered pedestrian doorsThe CE-marking takes into account the proof of conformity with the respective harmonized norms based on the legal provisions above.", "lang": "en"}, {"value": "Das KTV Atrium Flex Türenprogramm ist ein Durchbruch in Design mit Technologie: Die Karusselltür wird von einem elektromagnetischen Direktantrieb angetrieben – die dormakaba FLEX Direct Drive Technologie ergänzt den Designanspruch moderner Architektur. Es ist einzigartig, elegant und hinterlässt einen bleibenden und zeitlosen Eindruck.", "lang": "de"}]}, "quantitativeReference": {"referenceToReferenceFlow": [0]}, "time": {"referenceYear": 2023, "dataSetValidUntil": 2028, "other": {"anies": [{"name": "publicationDateOfEPD", "value": 1681430400000}]}}, "geography": {"locationOfOperationSupplyOrProduction": {"location": "GLO"}}, "technology": {"technologyDescriptionAndIncludedProcesses": [{"value": "The KTV Atrium Flex door range is a breakthrough in design with technology: The revolving door is driven by an electromagnetic direct drive - the dormakaba FLEX Direct Drive technology complements the design intent of modern architecture. It is unique, elegant and leaves an impression that is lasting and timeless. \nTechnical data: \nAdvanced German drive technology using innovative magnetic levitation technology, the door panels are directly driven by contactless magnetic fields, instead of conventional belt and gear system, realizing an extremely compact low-wear automation system that delivers quiet motion millions of times over. \nDeclared unit: \nThe declared unit is 1 piece of the product: KTV Atrium Flex", "lang": "en"}, {"value": "Die KTV Atrium Flex Türserie ist ein Durchbruch in Design und Technologie: Die Karusselltür wird durch einen elektromagnetischen Direktantrieb angetrieben - die dormakaba FLEX Direct Drive Technologie ergänzt den Gestaltungswillen der modernen Architektur. Sie ist einzigartig, elegant und hinterlässt einen bleibenden und zeitlosen Eindruck. \nTechnische Daten: \nDank der fortschrittlichen deutschen Antriebstechnologie mit innovativer Magnetschwebetechnik werden die Türflügel direkt durch berührungslose Magnetfelder angetrieben, anstelle eines konventionellen Riemen- und Getriebesystems. So wird ein extrem kompaktes, verschleißarmes Automatisierungssystem realisiert, das millionenfach leise Bewegungen ermöglicht. \nDeklarierte Einheit: \nDie angegebene Einheit ist 1 Stück des Produkts: KTV Atrium Flex", "lang": "de"}], "technologicalApplicability": [{"value": "The KTV Atrium Flex is ideal for modern entrances.\nTypical applications include:\n\nOffice / commercial buildings\nAirports\nPublic buildings\nHospitals\nHotels Automatic revolving doors are used to control the pedestrian flow in combination with an optimal thermal separation of the inside and outside climates during normal use.", "lang": "en"}, {"value": "Die KTV Atrium Flex ist ideal für moderne Eingänge. Typische Anwendungen sind: Büro-/Geschäftsgebäude Flughäfen Öffentliche Gebäude Krankenhäuser Hotels Automatische Karusselltüren werden zur Steuerung des Fußgängerstroms in Kombination mit einer optimalen thermischen Trennung des Innen- und Außenklimas bei normaler Nutzung eingesetzt.", "lang": "de"}]}}, "modellingAndValidation": {"LCIMethodAndAllocation": {"typeOfDataSet": "EPD", "referenceToLCAMethodDetails": [{"shortDescription": [{"value": "Automatic doors, automatic gates, and revolving door systems.pdf", "lang": "en"}], "type": "source data set", "refObjectId": "8573ccc5-f8cf-4e0e-9e9a-a5c3ed76d8fa"}], "other": {"anies": [{"name": "subType", "value": "specific dataset"}]}}, "dataSourcesTreatmentAndRepresentativeness": {"referenceToDataSource": [{"shortDescription": [{"value": "GaBi Database (all versions)", "lang": "en"}], "type": "source data set", "refObjectId": "28d74cc0-db8b-4d7e-bc44-5f6d56ce0c4a"}, {"shortDescription": [{"value": "GaBi database SP40 2020", "lang": "en"}], "type": "source data set", "refObjectId": "0115289e-52f0-4920-bc7e-57b1c96aec8d"}], "useAdviceForDataSet": [{"value": "Scope: \nThis Environmental Product Declaration refers to a specific KTV Atrium Flex All Glass Revolving Door manufactured by dormakaba. The production site is located in Sofia (Bulgaria). \n\nData represents the year 2022. \nSystem boundary: \nThe type of EPD is: cradle to gate with options, modules C1–C4, and module D (A1–A3 + C + D andadditional modules: A4 + A5 + B6)\n\nProduction - Module A1-A3\nThe product stage includes:\n— A1, raw material extraction, processing and mechanical treatments, processing of\nsecondarymaterial input (e.g. recycling processes),\n— A2, transport to the manufacturer,\n— A3, manufacturing and assemblyincluding provision of all materials, products and energy, as well as waste processing up to the end-of waste state.\n\nConstruction stage - Modules A4-A5\nThe construction process stage includes:\n— A4, transport to the building site;\n— A5, installation into the building; including provision of all materials, products and energy, as well as waste processing up to the end-ofwaste state or disposal of final residues during the construction process stage.\n\nUse stage - Module B6\nThe use stage related to the operation of the buildingincludes:\n— B6, operational energy use\n\nEnd-of-life stage– Modules C1-C4 and D\nThe end-of-life stage includes:\n— C1, de-construction, demolition:\n— C2, transport to waste processing;\n— C3, waste processing for reuse, recovery and/orrecycling;\n— C4, disposal; including provision and all transport, provision of all materials, products and related energy and water use.\nModule D (Benefits and loads beyond the system boundary) includes:\n— D, recycling potentials, expressed as net\nimpactsand benefits.", "lang": "en"}, {"value": "Gültigkeitsbereich: \nDiese Umweltproduktdeklaration bezieht sich auf eine bestimmte KTV Atrium Flex Ganzglas-Drehtür, die von dormakaba hergestellt wird. Die Produktionsstätte befindet sich in Sofia (Bulgarien). \n\nDie Daten beziehen sich auf das Jahr 2022. \nSystemgrenze: \nDie Art der EPD ist: Cradle to Gate mit Optionen, Modulen C1-C4 und Modul D (A1-A3 + C + D und zusätzliche Module: A4 + A5 + B6) Produktion - Modul A1-A3 Die Produktphase umfasst: - A1, Rohstoffgewinnung, Verarbeitung und mechanische Behandlungen, Verarbeitung von Sekundärmaterial-Input (z.B. Recyclingprozesse), - A2, Transport zum Hersteller, - A3, Herstellung und Montage einschließlich Bereitstellung aller Materialien, Produkte und Energie sowie Abfallverarbeitung bis zum End-of-Waste-Zustand.\n\nBauphase - Module A4-A5 Die Bauprozessphase umfasst: - A4, Transport zur Baustelle; - A5, Einbau in das Gebäude; einschließlich der Bereitstellung aller Materialien, Produkte und Energie sowie der Abfallverarbeitung bis zum Abfallende oder der Entsorgung der letzten Rückstände während der Bauprozessphase.\n\nNutzungsphase - Modul B6 Die Nutzungsphase im Zusammenhang mit dem Betrieb des Gebäudes umfasst: - B6, betrieblicher Energieverbrauch End-of-Life-Phase - Module C1-C4 und D Die End-of-Life-Phase umfasst: - C1, Rückbau, Abriss; - C2, Transport zur Abfallverarbeitung; - C3, Abfallverarbeitung zur Wiederverwendung, Verwertung und/oder zum Recycling; - C4, Entsorgung; einschließlich Bereitstellung und sämtlicher Transporte, Bereitstellung aller Materialien, Produkte und des damit verbundenen Energie- und Wasserverbrauchs.Modul D (Nutzen und Belastungen jenseits der Systemgrenze) umfasst: - D, Recyclingpotenziale, ausgedrückt als Nettoauswirkungen und -nutzen.", "lang": "de"}], "other": {"anies": [{"name": "referenceToOriginalEPD", "value": {"shortDescription": {"value": "KTV Atrium Flex.pdf", "defaultValue": "KTV Atrium Flex.pdf", "lstrings": [{"lang": "en", "value": "KTV Atrium Flex.pdf"}]}, "type": "source data set", "uuid": {"uuid": "854498f3-cf38-4d63-8ffb-fa86d974665f"}, "refObjectId": "854498f3-cf38-4d63-8ffb-fa86d974665f", "resourceURLs": ["https://oekobaudat.de/OEKOBAU.DAT/resource/sources/854498f3-cf38-4d63-8ffb-fa86d974665f/KTV_Atrium_Flex_22637.pdf?version=00.09.000"]}}]}}, "validation": {"review": [{"referenceToNameOfReviewerAndInstitution": [{"shortDescription": [{"value": "Institut Bauen und Umwelt e. V.", "lang": "en"}], "type": "contact data set", "refObjectId": "d111dbec-b024-4be5-86c5-752d6eb2cf95", "uri": "../contacts/d111dbec-b024-4be5-86c5-752d6eb2cf95.xml"}], "type": "Accredited third party review"}]}, "complianceDeclarations": {"compliance": [{"referenceToComplianceSystem": {"shortDescription": [{"value": "DIN EN 15804+A2", "lang": "en"}], "type": "source data set", "refObjectId": "c0016b33-8cf7-415c-ac6e-deba0d21440d", "uri": "../sources/c0016b33-8cf7-415c-ac6e-deba0d21440d.xml"}}, {"referenceToComplianceSystem": {"shortDescription": [{"value": "ISO 14025", "lang": "en"}], "type": "source data set", "refObjectId": "4f2eb655-6e44-4874-a95a-e28f5442cd4d", "uri": "../sources/4f2eb655-6e44-4874-a95a-e28f5442cd4d.xml"}}]}}, "administrativeInformation": {"commissionerAndGoal": {"referenceToCommissioner": [{"shortDescription": [{"value": "dormakaba International Holding GmbH", "lang": "en"}], "type": "contact data set", "refObjectId": "33313944-7b37-498a-b458-25a295c1017d", "uri": "../contacts/33313944-7b37-498a-b458-25a295c1017d.xml"}]}, "dataGenerator": {"referenceToPersonOrEntityGeneratingTheDataSet": [{"shortDescription": [{"value": "dormakaba International Holding GmbH", "lang": "en"}], "type": "contact data set", "refObjectId": "33313944-7b37-498a-b458-25a295c1017d", "uri": "../contacts/33313944-7b37-498a-b458-25a295c1017d.xml"}]}, "dataEntryBy": {"timeStamp": 1681430400000, "referenceToDataSetFormat": [{"shortDescription": [{"value": "ILCD Format", "lang": "en"}], "type": "source data set", "refObjectId": "a97a0155-0234-4b87-b4ce-a45da52f2a40", "uri": "../sources/a97a0155-0234-4b87-b4ce-a45da52f2a40.xml"}, {"shortDescription": [{"value": "EPD-Datenformaterweiterungen v1.2", "lang": "de"}, {"value": "EPD Data Format Extensions v1.2", "lang": "en"}], "type": "source data set", "refObjectId": "a29449fd-aa2f-4de8-b5d7-4b06b43c6fde", "uri": "../sources/a29449fd-aa2f-4de8-b5d7-4b06b43c6fde.xml"}]}, "publicationAndOwnership": {"dataSetVersion": "00.15.000", "referenceToRegistrationAuthority": {"shortDescription": [{"value": "Institut Bauen und Umwelt e. V.", "lang": "en"}], "type": "contact data set", "refObjectId": "d111dbec-b024-4be5-86c5-752d6eb2cf95", "uri": "../contacts/d111dbec-b024-4be5-86c5-752d6eb2cf95.xml"}, "registrationNumber": "EPD-DOR-20220356-CBA3-EN", "referenceToOwnershipOfDataSet": {"shortDescription": [{"value": "dormakaba International Holding GmbH", "lang": "en"}], "type": "contact data set", "refObjectId": "33313944-7b37-498a-b458-25a295c1017d", "uri": "../contacts/33313944-7b37-498a-b458-25a295c1017d.xml"}, "copyright": true, "licenseType": "Free of charge for all users and uses", "accessRestrictions": [{"value": "None", "lang": "en"}], "other": {"anies": [{"name": "referenceToPublisher", "value": {"shortDescription": [{"value": "Institut Bauen und Umwelt e. V.", "lang": "en"}], "type": "contact data set", "refObjectId": "d111dbec-b024-4be5-86c5-752d6eb2cf95", "uri": "../contacts/d111dbec-b024-4be5-86c5-752d6eb2cf95.xml"}}]}}}, "exchanges": {"exchange": [{"dataSetInternalID": 0, "referenceToFlowDataSet": {"shortDescription": [{"value": "KTV Atrium Flex (KTV Atrium Flex)", "lang": "en"}], "type": "flow data set", "refObjectId": "f5c39f1a-0ec4-c2ff-b8f9-31f491996207", "uri": "../flows/f5c39f1a-0ec4-c2ff-b8f9-31f491996207.xml"}, "meanAmount": 1.0, "referencesToDataSource": {}, "referenceFlow": true, "resolvedFlowVersion": "00.03.000", "resultingflowAmount": 6.6, "flowProperties": [{"name": [{"lang": "en", "value": "Area"}, {"lang": "de", "value": "Fläche"}], "uuid": "93a60a56-a3c8-19da-a746-0800200c9a66", "referenceFlowProperty": true, "meanValue": 6.6, "referenceUnit": "qm", "unitGroupUUID": "c20a03d7-bd90-4569-bc94-66cfd364dfc8"}, {"name": [{"lang": "en", "value": "Weight"}], "uuid": "93a60a56-a3c8-11da-a746-0800200b9a66", "meanValue": 1615.72}], "materialProperties": [{"name": "layer thickness", "value": "1.0", "unit": "m", "unitDescription": "meters"}, {"name": "grammage", "value": "244.8", "unit": "kg/m^2", "unitDescription": "kilograms per square meter"}], "typeOfFlow": "Product flow", "classification": {"classHierarchy": "Komponenten von Fenstern und Vorhangfassaden / Antriebssysteme / elektrisch", "name": "OEKOBAU.DAT"}}, {"dataSetInternalID": 1, "referenceToFlowDataSet": {"shortDescription": [{"value": "Renewable primary energy as energy carrier (PERE)", "lang": "en"}, {"value": "Erneuerbare Primärenergie als Energieträger (PERE)", "lang": "de"}], "type": "flow data set", "refObjectId": "20f32be5-0398-4288-9b6d-accddd195317", "uri": "../flows/20f32be5-0398-4288-9b6d-accddd195317.xml"}, "exchange direction": "INPUT", "other": {"anies": [{"name": "referenceToUnitGroupDataSet", "value": {"shortDescription": [{"value": "MJ", "lang": "en"}], "type": "unit group data set", "refObjectId": "93a60a57-a3c8-11da-a746-0800200c9a66", "uri": "../unitgroups/93a60a57-a3c8-11da-a746-0800200c9a66.xml"}}, {"value": "13676.587", "module": "A1-A3"}, {"value": "0.604", "module": "A4"}, {"value": "2106.8", "module": "A5"}, {"value": "11107", "module": "B6"}, {"value": "0", "module": "C1"}, {"value": "0.272", "module": "C2"}, {"value": "11.809", "module": "C3"}, {"value": "28.222", "module": "C4"}, {"value": "-7964.1", "module": "D"}]}, "resolvedFlowVersion": "38.00.000", "flowProperties": [], "typeOfFlow": "Other flow", "classification": {"classHierarchy": "Quantities", "name": "GaBiCategories"}}, {"dataSetInternalID": 2, "referenceToFlowDataSet": {"shortDescription": [{"value": "Renewable primary energy resources as material utilization (PERM)", "lang": "en"}, {"value": "Erneuerbare Primärenergie zur stofflichen Nutzung (PERM)", "lang": "de"}], "type": "flow data set", "refObjectId": "fb3ec0de-548d-4508-aea5-00b73bf6f702", "uri": "../flows/fb3ec0de-548d-4508-aea5-00b73bf6f702.xml"}, "exchange direction": "INPUT", "other": {"anies": [{"name": "referenceToUnitGroupDataSet", "value": {"shortDescription": [{"value": "MJ", "lang": "en"}], "type": "unit group data set", "refObjectId": "93a60a57-a3c8-11da-a746-0800200c9a66", "uri": "../unitgroups/93a60a57-a3c8-11da-a746-0800200c9a66.xml"}}, {"value": "2094.4", "module": "A1-A3"}, {"value": "0", "module": "A4"}, {"value": "-2094.4", "module": "A5"}, {"value": "0", "module": "B6"}, {"value": "0", "module": "C1"}, {"value": "0", "module": "C2"}, {"value": "0", "module": "C3"}, {"value": "0", "module": "C4"}, {"value": "0", "module": "D"}]}, "resolvedFlowVersion": "38.00.000", "flowProperties": [], "typeOfFlow": "Other flow", "classification": {"classHierarchy": "Quantities", "name": "GaBiCategories"}}, {"dataSetInternalID": 3, "referenceToFlowDataSet": {"shortDescription": [{"value": "Total use of renewable primary energy resources (PERT)", "lang": "en"}, {"value": "Total erneuerbare Primärenergie (PERT)", "lang": "de"}], "type": "flow data set", "refObjectId": "53f97275-fa8a-4cdd-9024-65936002acd0", "uri": "../flows/53f97275-fa8a-4cdd-9024-65936002acd0.xml"}, "exchange direction": "INPUT", "other": {"anies": [{"name": "referenceToUnitGroupDataSet", "value": {"shortDescription": [{"value": "MJ", "lang": "en"}], "type": "unit group data set", "refObjectId": "93a60a57-a3c8-11da-a746-0800200c9a66", "uri": "../unitgroups/93a60a57-a3c8-11da-a746-0800200c9a66.xml"}}, {"value": "15771.007", "module": "A1-A3"}, {"value": "0.604", "module": "A4"}, {"value": "12.418", "module": "A5"}, {"value": "11107", "module": "B6"}, {"value": "0", "module": "C1"}, {"value": "0.272", "module": "C2"}, {"value": "11.809", "module": "C3"}, {"value": "28.222", "module": "C4"}, {"value": "-7964.1", "module": "D"}]}, "resolvedFlowVersion": "38.00.000", "flowProperties": [], "typeOfFlow": "Other flow", "classification": {"classHierarchy": "Quantities / Environmental quantities / EPD EN 15804 / LCI indicators", "name": "GaBiCategories"}}, {"dataSetInternalID": 4, "referenceToFlowDataSet": {"shortDescription": [{"value": "Non renewable primary energy as energy carrier (PENRE)", "lang": "en"}, {"value": "Nicht-erneuerbare Primärenergie als Energieträger (PENRE)", "lang": "de"}], "type": "flow data set", "refObjectId": "ac857178-2b45-46ec-892a-a9a4332f0372", "uri": "../flows/ac857178-2b45-46ec-892a-a9a4332f0372.xml"}, "exchange direction": "INPUT", "other": {"anies": [{"name": "referenceToUnitGroupDataSet", "value": {"shortDescription": [{"value": "MJ", "lang": "en"}], "type": "unit group data set", "refObjectId": "93a60a57-a3c8-11da-a746-0800200c9a66", "uri": "../unitgroups/93a60a57-a3c8-11da-a746-0800200c9a66.xml"}}, {"value": "63730.2", "module": "A1-A3"}, {"value": "191.73", "module": "A4"}, {"value": "66.27", "module": "A5"}, {"value": "25064", "module": "B6"}, {"value": "0", "module": "C1"}, {"value": "86.205", "module": "C2"}, {"value": "1366.8", "module": "C3"}, {"value": "215.56", "module": "C4"}, {"value": "-22628", "module": "D"}]}, "resolvedFlowVersion": "38.00.000", "flowProperties": [], "typeOfFlow": "Other flow", "classification": {"classHierarchy": "Quantities", "name": "GaBiCategories"}}, {"dataSetInternalID": 5, "referenceToFlowDataSet": {"shortDescription": [{"value": "Non renewable primary energy as material utilization (PENRM)", "lang": "en"}, {"value": "Nicht-erneuerbare Primärenergie zur stofflichen Nutzung (PENRM)", "lang": "de"}], "type": "flow data set", "refObjectId": "1421caa0-679d-4bf4-b282-0eb850ccae27", "uri": "../flows/1421caa0-679d-4bf4-b282-0eb850ccae27.xml"}, "exchange direction": "INPUT", "other": {"anies": [{"name": "referenceToUnitGroupDataSet", "value": {"shortDescription": [{"value": "MJ", "lang": "en"}], "type": "unit group data set", "refObjectId": "93a60a57-a3c8-11da-a746-0800200c9a66", "uri": "../unitgroups/93a60a57-a3c8-11da-a746-0800200c9a66.xml"}}, {"value": "1321.3", "module": "A1-A3"}, {"value": "0", "module": "A4"}, {"value": "0", "module": "A5"}, {"value": "0", "module": "B6"}, {"value": "0", "module": "C1"}, {"value": "0", "module": "C2"}, {"value": "-1321.3", "module": "C3"}, {"value": "0", "module": "C4"}, {"value": "0", "module": "D"}]}, "resolvedFlowVersion": "38.00.000", "flowProperties": [], "typeOfFlow": "Other flow", "classification": {"classHierarchy": "Quantities", "name": "GaBiCategories"}}, {"dataSetInternalID": 6, "referenceToFlowDataSet": {"shortDescription": [{"value": "Total use of non renewable primary energy resources (PENRT)", "lang": "en"}, {"value": "Total nicht erneuerbare Primärenergie (PENRT)", "lang": "de"}], "type": "flow data set", "refObjectId": "06159210-646b-4c8d-8583-da9b3b95a6c1", "uri": "../flows/06159210-646b-4c8d-8583-da9b3b95a6c1.xml"}, "exchange direction": "INPUT", "other": {"anies": [{"name": "referenceToUnitGroupDataSet", "value": {"shortDescription": [{"value": "MJ", "lang": "en"}], "type": "unit group data set", "refObjectId": "93a60a57-a3c8-11da-a746-0800200c9a66", "uri": "../unitgroups/93a60a57-a3c8-11da-a746-0800200c9a66.xml"}}, {"value": "65052.2", "module": "A1-A3"}, {"value": "191.73", "module": "A4"}, {"value": "66.27", "module": "A5"}, {"value": "25064", "module": "B6"}, {"value": "0", "module": "C1"}, {"value": "86.205", "module": "C2"}, {"value": "45.419", "module": "C3"}, {"value": "215.56", "module": "C4"}, {"value": "-22628", "module": "D"}]}, "resolvedFlowVersion": "38.00.000", "flowProperties": [], "typeOfFlow": "Other flow", "classification": {"classHierarchy": "Quantities / Environmental quantities / EPD EN 15804 / LCI indicators", "name": "GaBiCategories"}}, {"dataSetInternalID": 7, "referenceToFlowDataSet": {"shortDescription": [{"value": "Use of secondary material (SM)", "lang": "en"}, {"value": "Einsatz von Sekundärstoffen (SM)", "lang": "de"}], "type": "flow data set", "refObjectId": "c6a1f35f-2d09-4f54-8dfb-97e502e1ce92", "uri": "../flows/c6a1f35f-2d09-4f54-8dfb-97e502e1ce92.xml"}, "exchange direction": "INPUT", "other": {"anies": [{"name": "referenceToUnitGroupDataSet", "value": {"shortDescription": [{"value": "kg", "lang": "en"}], "type": "unit group data set", "refObjectId": "ad38d542-3fe9-439d-9b95-2f5f7752acaf", "uri": "../unitgroups/ad38d542-3fe9-439d-9b95-2f5f7752acaf.xml"}}, {"value": "76.096", "module": "A1-A3"}, {"value": "0", "module": "A4"}, {"value": "0", "module": "A5"}, {"value": "0", "module": "B6"}, {"value": "0", "module": "C1"}, {"value": "0", "module": "C2"}, {"value": "0", "module": "C3"}, {"value": "0", "module": "C4"}, {"value": "0", "module": "D"}]}, "resolvedFlowVersion": "38.00.000", "flowProperties": [], "typeOfFlow": "Other flow", "classification": {"classHierarchy": "Quantities / Environmental quantities / EPD EN 15804 / LCI indicators", "name": "GaBiCategories"}}, {"dataSetInternalID": 8, "referenceToFlowDataSet": {"shortDescription": [{"value": "Use of renewable secondary fuels (RSF)", "lang": "en"}, {"value": "Erneuerbare Sekundärbrennstoffe (RSF)", "lang": "de"}], "type": "flow data set", "refObjectId": "64333088-a55f-4aa2-9a31-c10b07816787", "uri": "../flows/64333088-a55f-4aa2-9a31-c10b07816787.xml"}, "exchange direction": "INPUT", "other": {"anies": [{"name": "referenceToUnitGroupDataSet", "value": {"shortDescription": [{"value": "MJ", "lang": "en"}], "type": "unit group data set", "refObjectId": "93a60a57-a3c8-11da-a746-0800200c9a66", "uri": "../unitgroups/93a60a57-a3c8-11da-a746-0800200c9a66.xml"}}, {"value": "0", "module": "A1-A3"}, {"value": "0", "module": "A4"}, {"value": "0", "module": "A5"}, {"value": "0", "module": "B6"}, {"value": "0", "module": "C1"}, {"value": "0", "module": "C2"}, {"value": "0", "module": "C3"}, {"value": "0", "module": "C4"}, {"value": "0", "module": "D"}]}, "resolvedFlowVersion": "38.00.000", "flowProperties": [], "typeOfFlow": "Other flow", "classification": {"classHierarchy": "Quantities / Environmental quantities / EPD EN 15804 / LCI indicators", "name": "GaBiCategories"}}, {"dataSetInternalID": 9, "referenceToFlowDataSet": {"shortDescription": [{"value": "Use of non renewable secondary fuels (NRSF)", "lang": "en"}, {"value": "Nicht erneuerbare Sekundärbrennstoffe (NRSF)", "lang": "de"}], "type": "flow data set", "refObjectId": "89def144-d39a-4287-b86f-efde453ddcb2", "uri": "../flows/89def144-d39a-4287-b86f-efde453ddcb2.xml"}, "exchange direction": "INPUT", "other": {"anies": [{"name": "referenceToUnitGroupDataSet", "value": {"shortDescription": [{"value": "MJ", "lang": "en"}], "type": "unit group data set", "refObjectId": "93a60a57-a3c8-11da-a746-0800200c9a66", "uri": "../unitgroups/93a60a57-a3c8-11da-a746-0800200c9a66.xml"}}, {"value": "0", "module": "A1-A3"}, {"value": "0", "module": "A4"}, {"value": "0", "module": "A5"}, {"value": "0", "module": "B6"}, {"value": "0", "module": "C1"}, {"value": "0", "module": "C2"}, {"value": "0", "module": "C3"}, {"value": "0", "module": "C4"}, {"value": "0", "module": "D"}]}, "resolvedFlowVersion": "38.00.000", "flowProperties": [], "typeOfFlow": "Other flow", "classification": {"classHierarchy": "Quantities / Environmental quantities / EPD EN 15804 / LCI indicators", "name": "GaBiCategories"}}, {"dataSetInternalID": 10, "referenceToFlowDataSet": {"shortDescription": [{"value": "Use of net fresh water (FW)", "lang": "en"}, {"value": "Einsatz von Süßwasserressourcen (FW)", "lang": "de"}], "type": "flow data set", "refObjectId": "3cf952c8-f3a4-461d-8c96-96456ca62246", "uri": "../flows/3cf952c8-f3a4-461d-8c96-96456ca62246.xml"}, "exchange direction": "INPUT", "other": {"anies": [{"name": "referenceToUnitGroupDataSet", "value": {"shortDescription": [{"value": "m^3", "lang": "en"}], "type": "unit group data set", "refObjectId": "cd950537-0a98-4044-9ba7-9f9a68d0a504", "uri": "../unitgroups/cd950537-0a98-4044-9ba7-9f9a68d0a504.xml"}}, {"value": "45.673", "module": "A1-A3"}, {"value": "0.001", "module": "A4"}, {"value": "0.678", "module": "A5"}, {"value": "12.842", "module": "B6"}, {"value": "0", "module": "C1"}, {"value": "0.0004871", "module": "C2"}, {"value": "0.24", "module": "C3"}, {"value": "0.054", "module": "C4"}, {"value": "-21.423", "module": "D"}]}, "resolvedFlowVersion": "38.00.000", "flowProperties": [], "typeOfFlow": "Other flow", "classification": {"classHierarchy": "Quantities / Environmental quantities / EPD EN 15804 / LCI indicators", "name": "GaBiCategories"}}, {"dataSetInternalID": 11, "referenceToFlowDataSet": {"shortDescription": [{"value": "Hazardous waste disposed (HWD)", "lang": "en"}, {"value": "Gefährlicher Abfall zur Deponie (HWD)", "lang": "de"}], "type": "flow data set", "refObjectId": "430f9e0f-59b2-46a0-8e0d-55e0e84948fc", "uri": "../flows/430f9e0f-59b2-46a0-8e0d-55e0e84948fc.xml"}, "exchange direction": "OUTPUT", "other": {"anies": [{"name": "referenceToUnitGroupDataSet", "value": {"shortDescription": [{"value": "kg", "lang": "en"}], "type": "unit group data set", "refObjectId": "ad38d542-3fe9-439d-9b95-2f5f7752acaf", "uri": "../unitgroups/ad38d542-3fe9-439d-9b95-2f5f7752acaf.xml"}}, {"value": "0.0001461094", "module": "A1-A3"}, {"value": "1.86E-08", "module": "A4"}, {"value": "8.008E-08", "module": "A5"}, {"value": "1.037E-05", "module": "B6"}, {"value": "0", "module": "C1"}, {"value": "8.361E-09", "module": "C2"}, {"value": "1.731E-07", "module": "C3"}, {"value": "3.285E-06", "module": "C4"}, {"value": "-7.371E-05", "module": "D"}]}, "resolvedFlowVersion": "38.00.000", "flowProperties": [], "typeOfFlow": "Other flow", "classification": {"classHierarchy": "Quantities / Environmental quantities / EPD EN 15804 / LCI indicators", "name": "GaBiCategories"}}, {"dataSetInternalID": 12, "referenceToFlowDataSet": {"shortDescription": [{"value": "Non hazardous waste disposed (NHWD)", "lang": "en"}, {"value": "Entsorgter nicht gefährlicher Abfall (NHWD)", "lang": "de"}], "type": "flow data set", "refObjectId": "b29ef66b-e286-4afa-949f-62f1a7b4d7fa", "uri": "../flows/b29ef66b-e286-4afa-949f-62f1a7b4d7fa.xml"}, "exchange direction": "OUTPUT", "other": {"anies": [{"name": "referenceToUnitGroupDataSet", "value": {"shortDescription": [{"value": "kg", "lang": "en"}], "type": "unit group data set", "refObjectId": "ad38d542-3fe9-439d-9b95-2f5f7752acaf", "uri": "../unitgroups/ad38d542-3fe9-439d-9b95-2f5f7752acaf.xml"}}, {"value": "702.886", "module": "A1-A3"}, {"value": "0.02", "module": "A4"}, {"value": "5.161", "module": "A5"}, {"value": "17.781", "module": "B6"}, {"value": "0", "module": "C1"}, {"value": "0.009", "module": "C2"}, {"value": "10.173", "module": "C3"}, {"value": "1083.6", "module": "C4"}, {"value": "-293.79", "module": "D"}]}, "resolvedFlowVersion": "38.00.000", "flowProperties": [], "typeOfFlow": "Other flow", "classification": {"classHierarchy": "Quantities / Environmental quantities / EPD EN 15804 / LCI indicators", "name": "GaBiCategories"}}, {"dataSetInternalID": 13, "referenceToFlowDataSet": {"shortDescription": [{"value": "Radioactive waste disposed (RWD)", "lang": "en"}, {"value": "Entsorgter radioaktiver Abfall (RWD)", "lang": "de"}], "type": "flow data set", "refObjectId": "3449546e-52ad-4b39-b809-9fb77cea8ff6", "uri": "../flows/3449546e-52ad-4b39-b809-9fb77cea8ff6.xml"}, "exchange direction": "OUTPUT", "other": {"anies": [{"name": "referenceToUnitGroupDataSet", "value": {"shortDescription": [{"value": "kg", "lang": "en"}], "type": "unit group data set", "refObjectId": "ad38d542-3fe9-439d-9b95-2f5f7752acaf", "uri": "../unitgroups/ad38d542-3fe9-439d-9b95-2f5f7752acaf.xml"}}, {"value": "1.813", "module": "A1-A3"}, {"value": "0.0002058", "module": "A4"}, {"value": "0.004", "module": "A5"}, {"value": "3.803", "module": "B6"}, {"value": "0", "module": "C1"}, {"value": "9.253E-05", "module": "C2"}, {"value": "0.002", "module": "C3"}, {"value": "0.002", "module": "C4"}, {"value": "-1.574", "module": "D"}]}, "resolvedFlowVersion": "38.00.000", "flowProperties": [], "typeOfFlow": "Other flow", "classification": {"classHierarchy": "Quantities / Environmental quantities / EPD EN 15804 / LCI indicators", "name": "GaBiCategories"}}, {"dataSetInternalID": 14, "referenceToFlowDataSet": {"shortDescription": [{"value": "Components for re-use (CRU)", "lang": "en"}, {"value": "Komponenten für die Wiederverwendung (CRU)", "lang": "de"}], "type": "flow data set", "refObjectId": "a2b32f97-3fc7-4af2-b209-525bc6426f33", "uri": "../flows/a2b32f97-3fc7-4af2-b209-525bc6426f33.xml"}, "exchange direction": "OUTPUT", "other": {"anies": [{"name": "referenceToUnitGroupDataSet", "value": {"shortDescription": [{"value": "kg", "lang": "en"}], "type": "unit group data set", "refObjectId": "ad38d542-3fe9-439d-9b95-2f5f7752acaf", "uri": "../unitgroups/ad38d542-3fe9-439d-9b95-2f5f7752acaf.xml"}}, {"value": "0", "module": "A1-A3"}, {"value": "0", "module": "A4"}, {"value": "0", "module": "A5"}, {"value": "0", "module": "B6"}, {"value": "0", "module": "C1"}, {"value": "0", "module": "C2"}, {"value": "0", "module": "C3"}, {"value": "0", "module": "C4"}, {"value": "0", "module": "D"}]}, "resolvedFlowVersion": "38.00.000", "flowProperties": [], "typeOfFlow": "Other flow", "classification": {"classHierarchy": "Quantities / Environmental quantities / EPD EN 15804 / LCI indicators", "name": "GaBiCategories"}}, {"dataSetInternalID": 15, "referenceToFlowDataSet": {"shortDescription": [{"value": "Materials for recycling (MFR)", "lang": "en"}, {"value": "Stoffe zum Recycling (MFR)", "lang": "de"}], "type": "flow data set", "refObjectId": "d7fe48a5-4103-49c8-9aae-b0b5dfdbd6ae", "uri": "../flows/d7fe48a5-4103-49c8-9aae-b0b5dfdbd6ae.xml"}, "exchange direction": "OUTPUT", "other": {"anies": [{"name": "referenceToUnitGroupDataSet", "value": {"shortDescription": [{"value": "kg", "lang": "en"}], "type": "unit group data set", "refObjectId": "ad38d542-3fe9-439d-9b95-2f5f7752acaf", "uri": "../unitgroups/ad38d542-3fe9-439d-9b95-2f5f7752acaf.xml"}}, {"value": "0", "module": "A1-A3"}, {"value": "0", "module": "A4"}, {"value": "0", "module": "A5"}, {"value": "0", "module": "B6"}, {"value": "0", "module": "C1"}, {"value": "0", "module": "C2"}, {"value": "331.83", "module": "C3"}, {"value": "0", "module": "C4"}, {"value": "0", "module": "D"}]}, "resolvedFlowVersion": "38.00.000", "flowProperties": [], "typeOfFlow": "Other flow", "classification": {"classHierarchy": "Quantities / Environmental quantities / EPD EN 15804 / LCI indicators", "name": "GaBiCategories"}}, {"dataSetInternalID": 16, "referenceToFlowDataSet": {"shortDescription": [{"value": "Materials for energy recovery (MER)", "lang": "en"}, {"value": "Stoffe für die Energierückgewinnung (MER)", "lang": "de"}], "type": "flow data set", "refObjectId": "59a9181c-3aaf-46ee-8b13-2b3723b6e447", "uri": "../flows/59a9181c-3aaf-46ee-8b13-2b3723b6e447.xml"}, "exchange direction": "OUTPUT", "other": {"anies": [{"name": "referenceToUnitGroupDataSet", "value": {"shortDescription": [{"value": "kg", "lang": "en"}], "type": "unit group data set", "refObjectId": "ad38d542-3fe9-439d-9b95-2f5f7752acaf", "uri": "../unitgroups/ad38d542-3fe9-439d-9b95-2f5f7752acaf.xml"}}, {"value": "0", "module": "A1-A3"}, {"value": "0", "module": "A4"}, {"value": "0", "module": "A5"}, {"value": "0", "module": "B6"}, {"value": "0", "module": "C1"}, {"value": "0", "module": "C2"}, {"value": "0", "module": "C3"}, {"value": "0", "module": "C4"}, {"value": "0", "module": "D"}]}, "resolvedFlowVersion": "38.00.000", "flowProperties": [], "typeOfFlow": "Other flow", "classification": {"classHierarchy": "Quantities / Environmental quantities / EPD EN 15804 / LCI indicators", "name": "GaBiCategories"}}, {"dataSetInternalID": 17, "referenceToFlowDataSet": {"shortDescription": [{"value": "Exported electrical energy (EEE)", "lang": "en"}, {"value": "Exportierte elektrische Energie (EEE)", "lang": "de"}], "type": "flow data set", "refObjectId": "4da0c987-2b76-40d6-9e9e-82a017aaaf29", "uri": "../flows/4da0c987-2b76-40d6-9e9e-82a017aaaf29.xml"}, "exchange direction": "OUTPUT", "other": {"anies": [{"name": "referenceToUnitGroupDataSet", "value": {"shortDescription": [{"value": "MJ", "lang": "en"}], "type": "unit group data set", "refObjectId": "93a60a57-a3c8-11da-a746-0800200c9a66", "uri": "../unitgroups/93a60a57-a3c8-11da-a746-0800200c9a66.xml"}}, {"value": "0", "module": "A1-A3"}, {"value": "0", "module": "A4"}, {"value": "364.67", "module": "A5"}, {"value": "0", "module": "B6"}, {"value": "0", "module": "C1"}, {"value": "0", "module": "C2"}, {"value": "181.62", "module": "C3"}, {"value": "0", "module": "C4"}, {"value": "0", "module": "D"}]}, "resolvedFlowVersion": "38.00.000", "flowProperties": [], "typeOfFlow": "Other flow", "classification": {"classHierarchy": "Quantities / Environmental quantities / EPD EN 15804 / LCI indicators", "name": "GaBiCategories"}}, {"dataSetInternalID": 18, "referenceToFlowDataSet": {"shortDescription": [{"value": "Exported thermal energy (EET)", "lang": "en"}, {"value": "Exportierte thermische Energie (EET)", "lang": "de"}], "type": "flow data set", "refObjectId": "98daf38a-7a79-46d3-9a37-2b7bd0955810", "uri": "../flows/98daf38a-7a79-46d3-9a37-2b7bd0955810.xml"}, "exchange direction": "OUTPUT", "other": {"anies": [{"name": "referenceToUnitGroupDataSet", "value": {"shortDescription": [{"value": "MJ", "lang": "en"}], "type": "unit group data set", "refObjectId": "93a60a57-a3c8-11da-a746-0800200c9a66", "uri": "../unitgroups/93a60a57-a3c8-11da-a746-0800200c9a66.xml"}}, {"value": "0", "module": "A1-A3"}, {"value": "0", "module": "A4"}, {"value": "657.23", "module": "A5"}, {"value": "0", "module": "B6"}, {"value": "0", "module": "C1"}, {"value": "0", "module": "C2"}, {"value": "416.99", "module": "C3"}, {"value": "0", "module": "C4"}, {"value": "0", "module": "D"}]}, "resolvedFlowVersion": "38.00.000", "flowProperties": [], "typeOfFlow": "Other flow", "classification": {"classHierarchy": "Quantities / Environmental quantities / EPD EN 15804 / LCI indicators", "name": "GaBiCategories"}}]}, "LCIAResults": {"LCIAResult": [{"referenceToLCIAMethodDataSet": {"shortDescription": [{"value": "Global Warming Potential total (GWP-total)", "lang": "en"}, {"value": "Globales Erwärmungspotenzial total (GWP-total)", "lang": "de"}], "type": "LCIA method data set", "refObjectId": "6a37f984-a4b3-458a-a20a-64418c145fa2", "uri": "../lciamethods/6a37f984-a4b3-458a-a20a-64418c145fa2.xml"}, "other": {"anies": [{"name": "referenceToUnitGroupDataSet", "value": {"shortDescription": [{"value": "kg CO_(2) eq", "lang": "en"}], "type": "unit group data set", "refObjectId": "1ebf3012-d0db-4de2-aefd-ef30cedb0be1", "uri": "../unitgroups/1ebf3012-d0db-4de2-aefd-ef30cedb0be1.xml"}}, {"value": "4760.42", "module": "A1-A3"}, {"value": "14.132", "module": "A4"}, {"value": "261.99", "module": "A5"}, {"value": "1432.3", "module": "B6"}, {"value": "0", "module": "C1"}, {"value": "6.354", "module": "C2"}, {"value": "97.962", "module": "C3"}, {"value": "16.525", "module": "C4"}, {"value": "-1675.4", "module": "D"}]}}, {"referenceToLCIAMethodDataSet": {"shortDescription": [{"value": "Global Warming Potential fossil fuels (GWP-fossil)", "lang": "en"}, {"value": "Globales Erwärmungspotenzial fossil (GWP-fossil)", "lang": "de"}], "type": "LCIA method data set", "refObjectId": "5f635281-343e-44fb-83df-1971b155e6b6", "uri": "../lciamethods/5f635281-343e-44fb-83df-1971b155e6b6.xml"}, "other": {"anies": [{"name": "referenceToUnitGroupDataSet", "value": {"shortDescription": [{"value": "kg CO_(2) eq", "lang": "en"}], "type": "unit group data set", "refObjectId": "1ebf3012-d0db-4de2-aefd-ef30cedb0be1", "uri": "../unitgroups/1ebf3012-d0db-4de2-aefd-ef30cedb0be1.xml"}}, {"value": "4959.56", "module": "A1-A3"}, {"value": "13.507", "module": "A4"}, {"value": "4.862", "module": "A5"}, {"value": "1425.5", "module": "B6"}, {"value": "0", "module": "C1"}, {"value": "6.073", "module": "C2"}, {"value": "97.954", "module": "C3"}, {"value": "16.422", "module": "C4"}, {"value": "-1674.2", "module": "D"}]}}, {"referenceToLCIAMethodDataSet": {"shortDescription": [{"value": "Global Warming Potential biogenic (GWP-biogenic)", "lang": "en"}, {"value": "Globales Erwärmungspotenzial biogen (GWP-biogenic)", "lang": "de"}], "type": "LCIA method data set", "refObjectId": "2356e1ab-0185-4db5-86e5-16de51c7485c", "uri": "../lciamethods/2356e1ab-0185-4db5-86e5-16de51c7485c.xml"}, "other": {"anies": [{"name": "referenceToUnitGroupDataSet", "value": {"shortDescription": [{"value": "kg CO_(2) eq", "lang": "en"}], "type": "unit group data set", "refObjectId": "1ebf3012-d0db-4de2-aefd-ef30cedb0be1", "uri": "../unitgroups/1ebf3012-d0db-4de2-aefd-ef30cedb0be1.xml"}}, {"value": "-202.533", "module": "A1-A3"}, {"value": "0.624", "module": "A4"}, {"value": "257.13", "module": "A5"}, {"value": "4.752", "module": "B6"}, {"value": "0", "module": "C1"}, {"value": "0.281", "module": "C2"}, {"value": "0.002", "module": "C3"}, {"value": "0.056", "module": "C4"}, {"value": "0.299", "module": "D"}]}}, {"referenceToLCIAMethodDataSet": {"shortDescription": [{"value": "Global Warming Potential luluc (GWP-luluc)", "lang": "en"}, {"value": "Globales Erwärmungspotenzial luluc (GWP-luluc)", "lang": "de"}], "type": "LCIA method data set", "refObjectId": "4331bbdb-978a-490d-8707-eeb047f01a55", "uri": "../lciamethods/4331bbdb-978a-490d-8707-eeb047f01a55.xml"}, "other": {"anies": [{"name": "referenceToUnitGroupDataSet", "value": {"shortDescription": [{"value": "kg CO_(2) eq", "lang": "en"}], "type": "unit group data set", "refObjectId": "1ebf3012-d0db-4de2-aefd-ef30cedb0be1", "uri": "../unitgroups/1ebf3012-d0db-4de2-aefd-ef30cedb0be1.xml"}}, {"value": "3.461", "module": "A1-A3"}, {"value": "0.0003215", "module": "A4"}, {"value": "0.003", "module": "A5"}, {"value": "2.066", "module": "B6"}, {"value": "0", "module": "C1"}, {"value": "0.0001445", "module": "C2"}, {"value": "0.006", "module": "C3"}, {"value": "0.047", "module": "C4"}, {"value": "-1.52", "module": "D"}]}}, {"referenceToLCIAMethodDataSet": {"shortDescription": [{"value": "Depletion potential of the stratospheric ozone layer (ODP)", "lang": "en"}, {"value": "Abbau Potential der stratosphärischen Ozonschicht (ODP)", "lang": "de"}], "type": "LCIA method data set", "refObjectId": "b5c629d6-def3-11e6-bf01-fe55135034f3", "uri": "../lciamethods/b5c629d6-def3-11e6-bf01-fe55135034f3.xml"}, "other": {"anies": [{"name": "referenceToUnitGroupDataSet", "value": {"shortDescription": [{"value": "kg CFC11 eq", "lang": "en"}], "type": "unit group data set", "refObjectId": "d9e957c9-7309-4474-bf3a-7777df6c4e5b", "uri": "../unitgroups/d9e957c9-7309-4474-bf3a-7777df6c4e5b.xml"}}, {"value": "2.63032061E-09", "module": "A1-A3"}, {"value": "1.426E-15", "module": "A4"}, {"value": "3.833E-14", "module": "A5"}, {"value": "3.136E-11", "module": "B6"}, {"value": "0", "module": "C1"}, {"value": "6.411E-16", "module": "C2"}, {"value": "4.94E-14", "module": "C3"}, {"value": "6.089E-14", "module": "C4"}, {"value": "-6.919E-09", "module": "D"}]}}, {"referenceToLCIAMethodDataSet": {"shortDescription": [{"value": "Acidification potential of land and water (AP)", "lang": "en"}, {"value": "Versauerungspotenzial von Boden und Wasser (AP)", "lang": "de"}], "type": "LCIA method data set", "refObjectId": "b5c611c6-def3-11e6-bf01-fe55135034f3", "uri": "../lciamethods/b5c611c6-def3-11e6-bf01-fe55135034f3.xml"}, "other": {"anies": [{"name": "referenceToUnitGroupDataSet", "value": {"shortDescription": [{"value": "mol H^(+) eq", "lang": "en"}], "type": "unit group data set", "refObjectId": "42e089ac-92bf-4bf2-8ca1-5fc40d18f2ed", "uri": "../unitgroups/42e089ac-92bf-4bf2-8ca1-5fc40d18f2ed.xml"}}, {"value": "28.726", "module": "A1-A3"}, {"value": "0.014", "module": "A4"}, {"value": "0.044", "module": "A5"}, {"value": "3.147", "module": "B6"}, {"value": "0", "module": "C1"}, {"value": "0.006", "module": "C2"}, {"value": "0.017", "module": "C3"}, {"value": "0.118", "module": "C4"}, {"value": "-6.632", "module": "D"}]}}, {"referenceToLCIAMethodDataSet": {"shortDescription": [{"value": "Eutrophication potential aquatic freshwater (EP-freshwater)", "lang": "en"}, {"value": "Eutrophierungspotenzial Süßwasser (EP-freshwater)", "lang": "de"}], "type": "LCIA method data set", "refObjectId": "b53ec18f-7377-4ad3-86eb-cc3f4f276b2b", "uri": "../lciamethods/b53ec18f-7377-4ad3-86eb-cc3f4f276b2b.xml"}, "other": {"anies": [{"name": "referenceToUnitGroupDataSet", "value": {"shortDescription": [{"value": "kg P eq", "lang": "en"}], "type": "unit group data set", "refObjectId": "0429039d-a61d-4590-ba67-aa4a20a810a1", "uri": "../unitgroups/0429039d-a61d-4590-ba67-aa4a20a810a1.xml"}}, {"value": "0.00431088", "module": "A1-A3"}, {"value": "2.891E-06", "module": "A4"}, {"value": "6.718E-06", "module": "A5"}, {"value": "0.004", "module": "B6"}, {"value": "0", "module": "C1"}, {"value": "1.3E-06", "module": "C2"}, {"value": "7.879E-06", "module": "C3"}, {"value": "2.821E-05", "module": "C4"}, {"value": "-0.001", "module": "D"}]}}, {"referenceToLCIAMethodDataSet": {"shortDescription": [{"value": "Eutrophication potential aquatic marine (EP-marine)", "lang": "en"}, {"value": "Eutrophierungspotenzial Salzwasser (EP-marine)", "lang": "de"}], "type": "LCIA method data set", "refObjectId": "b5c619fa-def3-11e6-bf01-fe55135034f3", "uri": "../lciamethods/b5c619fa-def3-11e6-bf01-fe55135034f3.xml"}, "other": {"anies": [{"name": "referenceToUnitGroupDataSet", "value": {"shortDescription": [{"value": "kg N eq", "lang": "en"}], "type": "unit group data set", "refObjectId": "d05bb823-ecdf-4686-8c40-bf1d9257859f", "uri": "../unitgroups/d05bb823-ecdf-4686-8c40-bf1d9257859f.xml"}}, {"value": "5.664", "module": "A1-A3"}, {"value": "0.004", "module": "A4"}, {"value": "0.013", "module": "A5"}, {"value": "0.699", "module": "B6"}, {"value": "0", "module": "C1"}, {"value": "0.002", "module": "C2"}, {"value": "0.004", "module": "C3"}, {"value": "0.03", "module": "C4"}, {"value": "-0.949", "module": "D"}]}}, {"referenceToLCIAMethodDataSet": {"shortDescription": [{"value": "Eutrophication potential terrestrial (EP-terrestrial)", "lang": "en"}, {"value": "Eutrophierungspotenzial Land (EP-terrestrial)", "lang": "de"}], "type": "LCIA method data set", "refObjectId": "b5c614d2-def3-11e6-bf01-fe55135034f3", "uri": "../lciamethods/b5c614d2-def3-11e6-bf01-fe55135034f3.xml"}, "other": {"anies": [{"name": "referenceToUnitGroupDataSet", "value": {"shortDescription": [{"value": "mol N eq", "lang": "en"}], "type": "unit group data set", "refObjectId": "71b4d617-0ec9-4d3f-b65e-e438940c2401", "uri": "../unitgroups/71b4d617-0ec9-4d3f-b65e-e438940c2401.xml"}}, {"value": "63.488", "module": "A1-A3"}, {"value": "0.048", "module": "A4"}, {"value": "0.181", "module": "A5"}, {"value": "7.344", "module": "B6"}, {"value": "0", "module": "C1"}, {"value": "0.022", "module": "C2"}, {"value": "0.079", "module": "C3"}, {"value": "0.333", "module": "C4"}, {"value": "-10.288", "module": "D"}]}}, {"referenceToLCIAMethodDataSet": {"shortDescription": [{"value": "Formation potential of tropospheric ozone photochemical oxidants (POCP)", "lang": "en"}, {"value": "Bildungspotential für troposphärisches Ozon (POCP)", "lang": "de"}], "type": "LCIA method data set", "refObjectId": "b5c610fe-def3-11e6-bf01-fe55135034f3", "uri": "../lciamethods/b5c610fe-def3-11e6-bf01-fe55135034f3.xml"}, "other": {"anies": [{"name": "referenceToUnitGroupDataSet", "value": {"shortDescription": [{"value": "kg NMVOC eq", "lang": "en"}], "type": "unit group data set", "refObjectId": "d27c25f8-fbc1-44c6-b47b-4adbae4199c6", "uri": "../unitgroups/d27c25f8-fbc1-44c6-b47b-4adbae4199c6.xml"}}, {"value": "14.235", "module": "A1-A3"}, {"value": "0.012", "module": "A4"}, {"value": "0.035", "module": "A5"}, {"value": "1.915", "module": "B6"}, {"value": "0", "module": "C1"}, {"value": "0.005", "module": "C2"}, {"value": "0.011", "module": "C3"}, {"value": "0.092", "module": "C4"}, {"value": "-2.917", "module": "D"}]}}, {"referenceToLCIAMethodDataSet": {"shortDescription": [{"value": "Abiotic depletion potential for non fossil resources (ADPE)", "lang": "en"}, {"value": "Potenzial für den abiotischen Abbau nicht fossiler Ressourcen (ADPE)", "lang": "de"}], "type": "LCIA method data set", "refObjectId": "b2ad6494-c78d-11e6-9d9d-cec0c932ce01", "uri": "../lciamethods/b2ad6494-c78d-11e6-9d9d-cec0c932ce01.xml"}, "other": {"anies": [{"name": "referenceToUnitGroupDataSet", "value": {"shortDescription": [{"value": "kg Sb eq", "lang": "en"}], "type": "unit group data set", "refObjectId": "54ccd2d9-a32a-4fc2-923d-f2c8c93e89d4", "uri": "../unitgroups/54ccd2d9-a32a-4fc2-923d-f2c8c93e89d4.xml"}}, {"value": "0.07701431", "module": "A1-A3"}, {"value": "4.051E-07", "module": "A4"}, {"value": "6.064E-07", "module": "A5"}, {"value": "0.0004126", "module": "B6"}, {"value": "0", "module": "C1"}, {"value": "1.821E-07", "module": "C2"}, {"value": "6.775E-07", "module": "C3"}, {"value": "1.475E-06", "module": "C4"}, {"value": "-0.031", "module": "D"}]}}, {"referenceToLCIAMethodDataSet": {"shortDescription": [{"value": "Abiotic depletion potential for fossil resources (ADPF)", "lang": "en"}, {"value": "Potenzial für den abiotischen Abbau fossiler Brennstoffe (ADPF)", "lang": "de"}], "type": "LCIA method data set", "refObjectId": "b2ad6110-c78d-11e6-9d9d-cec0c932ce01", "uri": "../lciamethods/b2ad6110-c78d-11e6-9d9d-cec0c932ce01.xml"}, "other": {"anies": [{"name": "referenceToUnitGroupDataSet", "value": {"shortDescription": [{"value": "MJ", "lang": "en"}], "type": "unit group data set", "refObjectId": "93a60a57-a3c8-11da-a746-0800200c9a66", "uri": "../unitgroups/93a60a57-a3c8-11da-a746-0800200c9a66.xml"}}, {"value": "65021.9", "module": "A1-A3"}, {"value": "191.54", "module": "A4"}, {"value": "66.245", "module": "A5"}, {"value": "25059", "module": "B6"}, {"value": "0", "module": "C1"}, {"value": "86.121", "module": "C2"}, {"value": "45.407", "module": "C3"}, {"value": "215.46", "module": "C4"}, {"value": "-22611", "module": "D"}]}}, {"referenceToLCIAMethodDataSet": {"shortDescription": [{"value": "Water use (WDP)", "lang": "en"}, {"value": "Wassernutzung (WDP)", "lang": "de"}], "type": "LCIA method data set", "refObjectId": "b2ad66ce-c78d-11e6-9d9d-cec0c932ce01", "uri": "../lciamethods/b2ad66ce-c78d-11e6-9d9d-cec0c932ce01.xml"}, "other": {"anies": [{"name": "referenceToUnitGroupDataSet", "value": {"shortDescription": [{"value": "m^(3) world eq deprived", "lang": "en"}], "type": "unit group data set", "refObjectId": "6ae2df01-888e-46c8-b17d-49fa3869b476", "uri": "../unitgroups/6ae2df01-888e-46c8-b17d-49fa3869b476.xml"}}, {"value": "1092.92", "module": "A1-A3"}, {"value": "0.026", "module": "A4"}, {"value": "28.838", "module": "A5"}, {"value": "310.7", "module": "B6"}, {"value": "0", "module": "C1"}, {"value": "0.012", "module": "C2"}, {"value": "10.018", "module": "C3"}, {"value": "1.721", "module": "C4"}, {"value": "-328.23", "module": "D"}]}}, {"referenceToLCIAMethodDataSet": {"shortDescription": [{"value": "Incidence of disease due to PM emissions (PM)", "lang": "en"}, {"value": "Auftreten von Krankheiten aufgrund von Feinstaubemissionen (PM)", "lang": "de"}], "type": "LCIA method data set", "refObjectId": "b5c602c6-def3-11e6-bf01-fe55135034f3", "uri": "../lciamethods/b5c602c6-def3-11e6-bf01-fe55135034f3.xml"}, "other": {"anies": [{"name": "referenceToUnitGroupDataSet", "value": {"shortDescription": [{"value": "Disease incidence", "lang": "en"}], "type": "unit group data set", "refObjectId": "3883559b-648f-4afc-8ba2-0bd24f3affa3", "uri": "../unitgroups/3883559b-648f-4afc-8ba2-0bd24f3affa3.xml"}}, {"value": "0.000281318", "module": "A1-A3"}, {"value": "7.106E-08", "module": "A4"}, {"value": "2.987E-07", "module": "A5"}, {"value": "2.639E-05", "module": "B6"}, {"value": "0", "module": "C1"}, {"value": "3.195E-08", "module": "C2"}, {"value": "2.225E-07", "module": "C3"}, {"value": "1.458E-06", "module": "C4"}, {"value": "-0.000116", "module": "D"}]}}, {"referenceToLCIAMethodDataSet": {"shortDescription": [{"value": "Human exposure efficiency relative to U235 (IR)", "lang": "en"}, {"value": "Wirkung durch Exposition des Menschen mit U235 (IR)", "lang": "de"}], "type": "LCIA method data set", "refObjectId": "b5c632be-def3-11e6-bf01-fe55135034f3", "uri": "../lciamethods/b5c632be-def3-11e6-bf01-fe55135034f3.xml"}, "other": {"anies": [{"name": "referenceToUnitGroupDataSet", "value": {"shortDescription": [{"value": "kBq U235 eq", "lang": "en"}], "type": "unit group data set", "refObjectId": "456b05bf-1415-44a9-9993-02452f554c09", "uri": "../unitgroups/456b05bf-1415-44a9-9993-02452f554c09.xml"}}, {"value": "309.321", "module": "A1-A3"}, {"value": "0.029", "module": "A4"}, {"value": "0.578", "module": "A5"}, {"value": "623.96", "module": "B6"}, {"value": "0", "module": "C1"}, {"value": "0.013", "module": "C2"}, {"value": "0.152", "module": "C3"}, {"value": "0.252", "module": "C4"}, {"value": "-309.57", "module": "D"}]}}, {"referenceToLCIAMethodDataSet": {"shortDescription": [{"value": "Comparative toxic unit for ecosystems (ETP-fw)", "lang": "en"}, {"value": "Toxizitätsvergleichseinheit für Ökosysteme (ETP-fw)", "lang": "de"}], "type": "LCIA method data set", "refObjectId": "ee1082d1-b0f7-43ca-a1f0-21e2a4a74511", "uri": "../lciamethods/ee1082d1-b0f7-43ca-a1f0-21e2a4a74511.xml"}, "other": {"anies": [{"name": "referenceToUnitGroupDataSet", "value": {"shortDescription": [{"value": "CTUe", "lang": "en"}], "type": "unit group data set", "refObjectId": "aa959ded-f1eb-4efb-9c5c-2d60be36b3e6", "uri": "../unitgroups/aa959ded-f1eb-4efb-9c5c-2d60be36b3e6.xml"}}, {"value": "54043.9", "module": "A1-A3"}, {"value": "135.78", "module": "A4"}, {"value": "31.381", "module": "A5"}, {"value": "10720", "module": "B6"}, {"value": "0", "module": "C1"}, {"value": "61.049", "module": "C2"}, {"value": "17.043", "module": "C3"}, {"value": "123.1", "module": "C4"}, {"value": "-9368.2", "module": "D"}]}}, {"referenceToLCIAMethodDataSet": {"shortDescription": [{"value": "Comparative toxic unit for humans (carcinogenic) (HTP-c)", "lang": "en"}, {"value": "Toxizitätsvergleichseinheit für Menschen (krebserregend) (HTP-c)", "lang": "de"}], "type": "LCIA method data set", "refObjectId": "2299222a-bbd8-474f-9d4f-4dd1f18aea7c", "uri": "../lciamethods/2299222a-bbd8-474f-9d4f-4dd1f18aea7c.xml"}, "other": {"anies": [{"name": "referenceToUnitGroupDataSet", "value": {"shortDescription": [{"value": "CTUh", "lang": "en"}], "type": "unit group data set", "refObjectId": "d4c9523e-2d7e-49fd-8469-998f547d3a70", "uri": "../unitgroups/d4c9523e-2d7e-49fd-8469-998f547d3a70.xml"}}, {"value": "0.00021091775", "module": "A1-A3"}, {"value": "2.554E-09", "module": "A4"}, {"value": "2.399E-09", "module": "A5"}, {"value": "2.961E-07", "module": "B6"}, {"value": "0", "module": "C1"}, {"value": "1.148E-09", "module": "C2"}, {"value": "1.475E-09", "module": "C3"}, {"value": "1.824E-08", "module": "C4"}, {"value": "-1.6E-06", "module": "D"}]}}, {"referenceToLCIAMethodDataSet": {"shortDescription": [{"value": "Comparative toxic unit for humans (noncarcinogenic) (HTP-nc)", "lang": "en"}, {"value": "Toxizitätsvergleichseinheit für Menschen (nicht krebserregend) (HTP-nc)", "lang": "de"}], "type": "LCIA method data set", "refObjectId": "3af763a5-b7a1-48c9-9cee-1f223481fcef", "uri": "../lciamethods/3af763a5-b7a1-48c9-9cee-1f223481fcef.xml"}, "other": {"anies": [{"name": "referenceToUnitGroupDataSet", "value": {"shortDescription": [{"value": "CTUh", "lang": "en"}], "type": "unit group data set", "refObjectId": "d4c9523e-2d7e-49fd-8469-998f547d3a70", "uri": "../unitgroups/d4c9523e-2d7e-49fd-8469-998f547d3a70.xml"}}, {"value": "0.000134541", "module": "A1-A3"}, {"value": "1.092E-07", "module": "A4"}, {"value": "1.498E-07", "module": "A5"}, {"value": "1.091E-05", "module": "B6"}, {"value": "0", "module": "C1"}, {"value": "4.911E-08", "module": "C2"}, {"value": "1.494E-07", "module": "C3"}, {"value": "2.011E-06", "module": "C4"}, {"value": "-1.135E-05", "module": "D"}]}}, {"referenceToLCIAMethodDataSet": {"shortDescription": [{"value": "Soil quality index (SQP)", "lang": "en"}, {"value": "Bodenqualitätsindex (SQP)", "lang": "de"}], "type": "LCIA method data set", "refObjectId": "b2ad6890-c78d-11e6-9d9d-cec0c932ce01", "uri": "../lciamethods/b2ad6890-c78d-11e6-9d9d-cec0c932ce01.xml"}, "other": {"anies": [{"name": "referenceToUnitGroupDataSet", "value": {"shortDescription": [{"value": "SQP", "lang": "en"}], "type": "unit group data set", "refObjectId": "f130951c-e67f-4f7f-8dd4-665de3974e18", "uri": "../unitgroups/f130951c-e67f-4f7f-8dd4-665de3974e18.xml"}}, {"value": "38640.952", "module": "A1-A3"}, {"value": "0.492", "module": "A4"}, {"value": "18.368", "module": "A5"}, {"value": "7981", "module": "B6"}, {"value": "0", "module": "C1"}, {"value": "0.221", "module": "C2"}, {"value": "13.6", "module": "C3"}, {"value": "44.919", "module": "C4"}, {"value": "-1923.8", "module": "D"}]}}]}, "otherAttributes": {"{http://www.indata.network/EPD/2019}epd-version": "1.2"}, "version": "1.1", "locations": "../ILCDLocations.xml"}