{"processInformation": {"dataSetInformation": {"UUID": "b4f4c301-0af1-4e63-ad99-abe83ef3c221", "name": {"baseName": [{"value": "Welded and painted steel structures: Other steel structures (Heidelberg Materials SBC Latvia SIA)", "lang": "en"}, {"value": "Geschweißte und lackierte Stahlkonstruktionen: Sonstige Stahlkonstruktionen (Heidelberg Materials SBC Latvia SIA)", "lang": "de"}]}, "synonyms": [{"value": "Welded and painted steel structures (Heidelberg Materials SBC Latvia SIA)", "lang": "en"}], "classificationInformation": {"classification": [{"class": [{"value": "Metalle", "level": 0, "classId": "4"}, {"value": "Stahl und Eisen", "level": 1, "classId": "4.1"}, {"value": "Stahlprofile", "level": 2, "classId": "4.1.03"}], "name": "OEKOBAU.DAT"}]}, "generalComment": [{"value": "The EPD (type: Cradle to gate with options, modules C1-C4 and module D (A1-A4, C, D)) is based on LCA of the custom made welded and painted steel structures (box beams and other structures), manufactured in Mārupe, Latvia. The calculation is based on 1 metric ton of welded and surface treated steel structure with a share of 98,4% (box beams) and 98,8% (other structures) steel materials. Kiwa-Ecobility Experts shall not be liable with respect to manufacturer information, life cycle assessment data and evidence.", "lang": "en"}], "other": {"anies": [{"scenario": [{"description": [{"value": "All installed raw materials of the product were analysed, and the masses were determined following the allocation and cut-off requirements. Production-specific energy consumption was measured and provided by Heidelberg Materials SBC Latvia SIA. Since the production process is quite similar for all of steel products produced at the manufacturing site, the energy consumption, ancillary materials, and production waste were appropriated according to the annual use of steel materials and then declared per 1 metric ton of the products. The total annual production data is recorded to a high standard of accuracy and precision. The production waste is collected separately. As the product is marketed internationally, no country-specific waste scenario can be considered. Therefore, the waste scenarios of NMD (2022) were adopted.", "lang": "en"}], "name": "Standard Scenario", "default": true}, {"name": "Sweden Scenario", "default": false}, {"name": "Norway Scenario", "default": false}]}, "<ns11:modules xmlns:ns11=\"http://openlca.org/epd_ilcd\" xmlns=\"http://lca.jrc.it/ILCD/Process\" xmlns:c=\"http://lca.jrc.it/ILCD/Contact\" xmlns:common=\"http://lca.jrc.it/ILCD/Common\" xmlns:epd=\"http://www.iai.kit.edu/EPD/2013\" xmlns:epd2=\"http://www.indata.network/EPD/2019\" xmlns:f=\"http://lca.jrc.it/ILCD/Flow\" xmlns:fp=\"http://lca.jrc.it/ILCD/FlowProperty\" xmlns:m=\"http://lca.jrc.it/ILCD/LCIAMethod\" xmlns:s=\"http://lca.jrc.it/ILCD/Source\" xmlns:u=\"http://lca.jrc.it/ILCD/UnitGroup\" name=\"A1\" scenario=\"Standard Scenario\"/>", "<ns11:modules xmlns:ns11=\"http://openlca.org/epd_ilcd\" xmlns=\"http://lca.jrc.it/ILCD/Process\" xmlns:c=\"http://lca.jrc.it/ILCD/Contact\" xmlns:common=\"http://lca.jrc.it/ILCD/Common\" xmlns:epd=\"http://www.iai.kit.edu/EPD/2013\" xmlns:epd2=\"http://www.indata.network/EPD/2019\" xmlns:f=\"http://lca.jrc.it/ILCD/Flow\" xmlns:fp=\"http://lca.jrc.it/ILCD/FlowProperty\" xmlns:m=\"http://lca.jrc.it/ILCD/LCIAMethod\" xmlns:s=\"http://lca.jrc.it/ILCD/Source\" xmlns:u=\"http://lca.jrc.it/ILCD/UnitGroup\" name=\"A2\" scenario=\"Standard Scenario\"/>", "<ns11:modules xmlns:ns11=\"http://openlca.org/epd_ilcd\" xmlns=\"http://lca.jrc.it/ILCD/Process\" xmlns:c=\"http://lca.jrc.it/ILCD/Contact\" xmlns:common=\"http://lca.jrc.it/ILCD/Common\" xmlns:epd=\"http://www.iai.kit.edu/EPD/2013\" xmlns:epd2=\"http://www.indata.network/EPD/2019\" xmlns:f=\"http://lca.jrc.it/ILCD/Flow\" xmlns:fp=\"http://lca.jrc.it/ILCD/FlowProperty\" xmlns:m=\"http://lca.jrc.it/ILCD/LCIAMethod\" xmlns:s=\"http://lca.jrc.it/ILCD/Source\" xmlns:u=\"http://lca.jrc.it/ILCD/UnitGroup\" name=\"A3\" scenario=\"Standard Scenario\"/>", "<ns11:modules xmlns:ns11=\"http://openlca.org/epd_ilcd\" xmlns=\"http://lca.jrc.it/ILCD/Process\" xmlns:c=\"http://lca.jrc.it/ILCD/Contact\" xmlns:common=\"http://lca.jrc.it/ILCD/Common\" xmlns:epd=\"http://www.iai.kit.edu/EPD/2013\" xmlns:epd2=\"http://www.indata.network/EPD/2019\" xmlns:f=\"http://lca.jrc.it/ILCD/Flow\" xmlns:fp=\"http://lca.jrc.it/ILCD/FlowProperty\" xmlns:m=\"http://lca.jrc.it/ILCD/LCIAMethod\" xmlns:s=\"http://lca.jrc.it/ILCD/Source\" xmlns:u=\"http://lca.jrc.it/ILCD/UnitGroup\" name=\"A4\" scenario=\"Norway Scenario\"/>", "<ns11:modules xmlns:ns11=\"http://openlca.org/epd_ilcd\" xmlns=\"http://lca.jrc.it/ILCD/Process\" xmlns:c=\"http://lca.jrc.it/ILCD/Contact\" xmlns:common=\"http://lca.jrc.it/ILCD/Common\" xmlns:epd=\"http://www.iai.kit.edu/EPD/2013\" xmlns:epd2=\"http://www.indata.network/EPD/2019\" xmlns:f=\"http://lca.jrc.it/ILCD/Flow\" xmlns:fp=\"http://lca.jrc.it/ILCD/FlowProperty\" xmlns:m=\"http://lca.jrc.it/ILCD/LCIAMethod\" xmlns:s=\"http://lca.jrc.it/ILCD/Source\" xmlns:u=\"http://lca.jrc.it/ILCD/UnitGroup\" name=\"A4\" scenario=\"Sweden Scenario\"/>", "<ns11:modules xmlns:ns11=\"http://openlca.org/epd_ilcd\" xmlns=\"http://lca.jrc.it/ILCD/Process\" xmlns:c=\"http://lca.jrc.it/ILCD/Contact\" xmlns:common=\"http://lca.jrc.it/ILCD/Common\" xmlns:epd=\"http://www.iai.kit.edu/EPD/2013\" xmlns:epd2=\"http://www.indata.network/EPD/2019\" xmlns:f=\"http://lca.jrc.it/ILCD/Flow\" xmlns:fp=\"http://lca.jrc.it/ILCD/FlowProperty\" xmlns:m=\"http://lca.jrc.it/ILCD/LCIAMethod\" xmlns:s=\"http://lca.jrc.it/ILCD/Source\" xmlns:u=\"http://lca.jrc.it/ILCD/UnitGroup\" name=\"C1\" scenario=\"Standard Scenario\"/>", "<ns11:modules xmlns:ns11=\"http://openlca.org/epd_ilcd\" xmlns=\"http://lca.jrc.it/ILCD/Process\" xmlns:c=\"http://lca.jrc.it/ILCD/Contact\" xmlns:common=\"http://lca.jrc.it/ILCD/Common\" xmlns:epd=\"http://www.iai.kit.edu/EPD/2013\" xmlns:epd2=\"http://www.indata.network/EPD/2019\" xmlns:f=\"http://lca.jrc.it/ILCD/Flow\" xmlns:fp=\"http://lca.jrc.it/ILCD/FlowProperty\" xmlns:m=\"http://lca.jrc.it/ILCD/LCIAMethod\" xmlns:s=\"http://lca.jrc.it/ILCD/Source\" xmlns:u=\"http://lca.jrc.it/ILCD/UnitGroup\" name=\"C2\" scenario=\"Standard Scenario\"/>", "<ns11:modules xmlns:ns11=\"http://openlca.org/epd_ilcd\" xmlns=\"http://lca.jrc.it/ILCD/Process\" xmlns:c=\"http://lca.jrc.it/ILCD/Contact\" xmlns:common=\"http://lca.jrc.it/ILCD/Common\" xmlns:epd=\"http://www.iai.kit.edu/EPD/2013\" xmlns:epd2=\"http://www.indata.network/EPD/2019\" xmlns:f=\"http://lca.jrc.it/ILCD/Flow\" xmlns:fp=\"http://lca.jrc.it/ILCD/FlowProperty\" xmlns:m=\"http://lca.jrc.it/ILCD/LCIAMethod\" xmlns:s=\"http://lca.jrc.it/ILCD/Source\" xmlns:u=\"http://lca.jrc.it/ILCD/UnitGroup\" name=\"C3\" scenario=\"Standard Scenario\"/>", "<ns11:modules xmlns:ns11=\"http://openlca.org/epd_ilcd\" xmlns=\"http://lca.jrc.it/ILCD/Process\" xmlns:c=\"http://lca.jrc.it/ILCD/Contact\" xmlns:common=\"http://lca.jrc.it/ILCD/Common\" xmlns:epd=\"http://www.iai.kit.edu/EPD/2013\" xmlns:epd2=\"http://www.indata.network/EPD/2019\" xmlns:f=\"http://lca.jrc.it/ILCD/Flow\" xmlns:fp=\"http://lca.jrc.it/ILCD/FlowProperty\" xmlns:m=\"http://lca.jrc.it/ILCD/LCIAMethod\" xmlns:s=\"http://lca.jrc.it/ILCD/Source\" xmlns:u=\"http://lca.jrc.it/ILCD/UnitGroup\" name=\"C4\" scenario=\"Standard Scenario\"/>", "<ns11:modules xmlns:ns11=\"http://openlca.org/epd_ilcd\" xmlns=\"http://lca.jrc.it/ILCD/Process\" xmlns:c=\"http://lca.jrc.it/ILCD/Contact\" xmlns:common=\"http://lca.jrc.it/ILCD/Common\" xmlns:epd=\"http://www.iai.kit.edu/EPD/2013\" xmlns:epd2=\"http://www.indata.network/EPD/2019\" xmlns:f=\"http://lca.jrc.it/ILCD/Flow\" xmlns:fp=\"http://lca.jrc.it/ILCD/FlowProperty\" xmlns:m=\"http://lca.jrc.it/ILCD/LCIAMethod\" xmlns:s=\"http://lca.jrc.it/ILCD/Source\" xmlns:u=\"http://lca.jrc.it/ILCD/UnitGroup\" name=\"D\" scenario=\"Standard Scenario\"/>"]}}, "quantitativeReference": {"referenceToReferenceFlow": [1], "type": "Reference flow(s)"}, "time": {"referenceYear": 2022, "dataSetValidUntil": 2029, "timeRepresentativenessDescription": [{"value": "The reference year for collecting data is 2022 (01.2022 – 12.2022).", "lang": "en"}], "other": {"anies": [{"name": "publicationDateOfEPD", "value": 1704758400000}]}}, "geography": {"locationOfOperationSupplyOrProduction": {"descriptionOfRestrictions": [{"value": "The geographical reference area is Europe or Global and can be seen in the System description boundary table.", "lang": "en"}], "location": "RER"}}, "technology": {"technologyDescriptionAndIncludedProcesses": [{"value": "Welded and painted steel structures are customized construction components for many applications, including load-bearing and non-load bearing structures, used in every type of building, including, industrial buildings, agricultural buildings, commercial buildings. The steel structures are manufactured according to EN 1090-2, up to EXC 4, and are CE- marked. UN CPC code: 421 Structural metal products and parts thereof.\r\nThe steel structures of industrial and civil objects from SIA Heidelberg Materials SBC Latvia are made according to drawings. The manufacturing route contains the following processes: \r\n- Extraction and delivery of raw materials; - Cutting (plasma cutting, sawing, drilling etc.); - Assembling; - Welding; - Shot blasting; - Coating;  - Storage; - Transportation (delivery of finished products)\r\n", "lang": "en"}], "technologicalApplicability": [{"value": "The products are prefabricated elements and are intended to be used as part of building (e.g. columns, beams, trusses, connections) or various auxiliary instalments like bridge, pylon, structures, indoor and outdoor stairs and other construction elements.", "lang": "en"}], "referenceToTechnologyFlowDiagrammOrPicture": [{"shortDescription": [{"value": "Flow Chart for Welded and painted steel structures (Heidelberg Materials SBC Latvia SIA)", "lang": "en"}], "type": "source data set", "refObjectId": "11152f76-1bea-48f3-9fb1-e1819360d1a9", "version": "00.00.001"}]}}, "modellingAndValidation": {"LCIMethodAndAllocation": {"typeOfDataSet": "EPD", "other": {"anies": [{"name": "subType", "value": "average dataset"}]}}, "dataSourcesTreatmentAndRepresentativeness": {"referenceToDataSource": [{"shortDescription": [{"value": "ecoinvent database (general)", "lang": "en"}], "type": "source data set", "refObjectId": "b497a91f-e14b-4b69-8f28-f50eb1576766", "version": "00.03.002"}, {"shortDescription": [{"value": "ecoinvent 3.6 database", "lang": "en"}], "type": "source data set", "refObjectId": "766b9973-5ee8-48a2-8098-72c8e20b369f", "version": "00.00.001"}], "useAdviceForDataSet": [{"value": "The products are prefabricated elements and are intended to be used as part of building (e.g. columns, beams, trusses, connections) or various auxiliary instalments like bridge, pylon, structures, indoor and outdoor stairs and other construction elements.", "lang": "en"}], "other": {"anies": [{"name": "referenceToOriginalEPD", "value": {"shortDescription": {"value": "EPD for Welded and painted steel structures (Heidelberg Materials SBC Latvia SIA)", "defaultValue": "EPD for Welded and painted steel structures (Heidelberg Materials SBC Latvia SIA)", "lstrings": [{"lang": "en", "value": "EPD for Welded and painted steel structures (Heidelberg Materials SBC Latvia SIA)"}]}, "version": {"version": 1, "majorVersion": 0, "minorVersion": 0, "subMinorVersion": 1, "zero": false, "versionString": "00.00.001"}, "type": "source data set", "uuid": {"uuid": "c4fa8fe7-aff5-4777-8fe7-9c6c31721409"}, "refObjectId": "c4fa8fe7-aff5-4777-8fe7-9c6c31721409", "versionAsString": "00.00.001", "resourceURLs": ["https://oekobaudat.de/OEKOBAU.DAT/resource/sources/c4fa8fe7-aff5-4777-8fe7-9c6c31721409/EPD-Kiwa-EE-000368-EN.pdf?version=00.00.001"]}}]}}, "validation": {"review": [{"reviewDetails": [{"value": "Independent verification of the declaration and data according to ISO 14025:2010.", "lang": "en"}], "referenceToNameOfReviewerAndInstitution": [{"shortDescription": [{"value": "Elisabet Amat Guasch (External verifier)", "lang": "en"}], "type": "contact data set", "refObjectId": "50fe5785-3ff2-46e5-935a-dab7a249bab3", "version": "00.00.001"}], "type": "Independent external review"}]}, "complianceDeclarations": {"compliance": [{"referenceToComplianceSystem": {"shortDescription": [{"value": "ISO 14025", "lang": "en"}], "type": "source data set", "refObjectId": "4f2eb655-6e44-4874-a95a-e28f5442cd4d", "version": "00.00.001"}}, {"referenceToComplianceSystem": {"shortDescription": [{"value": "EN 15804+A2 (EF 3.0)", "lang": "de"}, {"value": "EN 15804+A2 (EF 3.0)", "lang": "en"}], "type": "source data set", "refObjectId": "c0016b33-8cf7-415c-ac6e-deba0d21440d", "version": "00.02.000"}}]}}, "administrativeInformation": {"commissionerAndGoal": {"referenceToCommissioner": [{"shortDescription": [{"value": "Heidelberg Materials SBC Latvia SIA", "lang": "en"}], "type": "contact data set", "refObjectId": "635b13ba-f8f1-45ef-af8a-ea693dd12991", "version": "00.00.001"}]}, "dataGenerator": {"referenceToPersonOrEntityGeneratingTheDataSet": [{"shortDescription": [{"value": "Kiwa GmbH (Berlin)", "lang": "en"}], "type": "contact data set", "refObjectId": "3ea4a87a-3f88-4633-b7e7-1bbdd272be43", "version": "00.00.002"}]}, "dataEntryBy": {"timeStamp": 1752581588023, "referenceToDataSetFormat": [{"shortDescription": [{"value": "ILCD format", "lang": "en"}], "type": "source data set", "refObjectId": "a97a0155-0234-4b87-b4ce-a45da52f2a40", "version": "01.00.000", "uri": "http://lca.jrc.ec.europa.eu/lcainfohub/sample_data/ilcd/sources/ILCD_Format_a97a0155-0234-4b87-b4ce-a45da52f2a40_01.00.000.xml"}, {"shortDescription": [{"value": "EPD Data Format Extensions v1.2", "lang": "en"}, {"value": "EPD-Datenformaterweiterungen v1.2", "lang": "de"}], "type": "source data set", "refObjectId": "a29449fd-aa2f-4de8-b5d7-4b06b43c6fde", "version": "00.01.000"}], "referenceToPersonOrEntityEnteringTheData": {"shortDescription": [{"value": "Kiwa GmbH (Berlin)", "lang": "en"}], "type": "contact data set", "refObjectId": "3ea4a87a-3f88-4633-b7e7-1bbdd272be43", "version": "00.00.002"}}, "publicationAndOwnership": {"dataSetVersion": "00.00.016", "referenceToRegistrationAuthority": {"shortDescription": [{"value": "Kiwa-Ecobility Experts, Kiwa GmbH (Berlin)", "lang": "en"}], "type": "contact data set", "refObjectId": "eb52a9a8-9d0f-40ce-a5c9-7b78f5615e5a", "version": "00.00.002"}, "registrationNumber": "EPD-Kiwa-EE-000368-EN", "referenceToOwnershipOfDataSet": {"shortDescription": [{"value": "Heidelberg Materials SBC Latvia SIA", "lang": "en"}], "type": "contact data set", "refObjectId": "635b13ba-f8f1-45ef-af8a-ea693dd12991", "version": "00.00.001"}, "copyright": true, "licenseType": "Free of charge for all users and uses", "accessRestrictions": [{"value": "None", "lang": "en"}], "other": {"anies": [{"name": "referenceToPublisher", "value": {"shortDescription": [{"value": "Kiwa-Ecobility Experts, Kiwa GmbH (Berlin)", "lang": "en"}], "type": "contact data set", "refObjectId": "eb52a9a8-9d0f-40ce-a5c9-7b78f5615e5a", "version": "00.00.002"}}]}}}, "exchanges": {"exchange": [{"dataSetInternalID": 1, "referenceToFlowDataSet": {"shortDescription": [{"value": "Welded and painted steel structures (Heidelberg Materials SBC Latvia SIA)", "lang": "en"}], "type": "flow data set", "refObjectId": "9ebbc4de-9df2-448d-a4c5-af5b0e43a293", "version": "00.00.003"}, "meanAmount": 1.0, "resultingAmount": 1.0, "referenceFlow": true, "resultingflowAmount": 1000.0, "flowProperties": [{"name": [{"lang": "en", "value": "Mass"}, {"lang": "de", "value": "Masse"}], "uuid": "93a60a56-a3c8-11da-a746-0800200b9a66", "referenceFlowProperty": true, "meanValue": 1000.0, "referenceUnit": "kg", "unitGroupUUID": "ad38d542-3fe9-439d-9b95-2f5f7752acaf"}], "materialProperties": [{"name": "gross density", "value": "7850.0", "unit": "kg/m^3", "unitDescription": "kilograms per cubic metre"}], "typeOfFlow": "Product flow", "classification": {"classHierarchy": "Metalle / Stahl und Eisen / Stahlprofile", "name": "OEKOBAU.DAT"}}, {"dataSetInternalID": 2, "referenceToFlowDataSet": {"shortDescription": [{"value": "Components for re-use (CRU)", "lang": "en"}, {"value": "Komponenten für die Wiederverwendung (CRU)", "lang": "de"}, {"value": "Componentes para su reutilización (CRU)", "lang": "es"}], "type": "flow data set", "refObjectId": "a2b32f97-3fc7-4af2-b209-525bc6426f33", "version": "30.00.000", "uri": "../flows/a2b32f97-3fc7-4af2-b209-525bc6426f33.xml"}, "exchange direction": "OUTPUT", "meanAmount": 0.0, "other": {"anies": [{"value": "0.0", "module": "A1", "scenario": "Standard Scenario"}, {"value": "0.0", "module": "A2", "scenario": "Standard Scenario"}, {"value": "0.0", "module": "A3", "scenario": "Standard Scenario"}, {"value": "0.0", "module": "A4", "scenario": "Norway Scenario"}, {"value": "0.0", "module": "A4", "scenario": "Sweden Scenario"}, {"value": "0.0", "module": "C1", "scenario": "Standard Scenario"}, {"value": "0.0", "module": "C2", "scenario": "Standard Scenario"}, {"value": "50.0", "module": "C3", "scenario": "Standard Scenario"}, {"value": "0.0", "module": "C4", "scenario": "Standard Scenario"}, {"value": "0.0", "module": "D", "scenario": "Standard Scenario"}, {"name": "referenceToUnitGroupDataSet", "value": {"shortDescription": [{"value": "kg", "lang": "en"}], "type": "unit group data set", "refObjectId": "ad38d542-3fe9-439d-9b95-2f5f7752acaf", "version": "30.00.000", "uri": "../unitgroups/ad38d542-3fe9-439d-9b95-2f5f7752acaf.xml"}}]}, "flowProperties": [], "typeOfFlow": "Other flow", "classification": {"classHierarchy": "Größen / Umweltliche Größen / EPD EN 15804 / LCI Indikatoren", "name": "GaBiCategories"}}, {"dataSetInternalID": 3, "referenceToFlowDataSet": {"shortDescription": [{"value": "Exported electrical energy (EEE)", "lang": "en"}, {"value": "Exportierte elektrische Energie (EEE)", "lang": "de"}, {"value": "Energía exportada electrica (EEE)", "lang": "es"}], "type": "flow data set", "refObjectId": "4da0c987-2b76-40d6-9e9e-82a017aaaf29", "version": "30.00.000", "uri": "../flows/4da0c987-2b76-40d6-9e9e-82a017aaaf29.xml"}, "exchange direction": "OUTPUT", "meanAmount": 0.0, "other": {"anies": [{"value": "0.0", "module": "A1", "scenario": "Standard Scenario"}, {"value": "0.0", "module": "A2", "scenario": "Standard Scenario"}, {"value": "0.0", "module": "A3", "scenario": "Standard Scenario"}, {"value": "0.0", "module": "A4", "scenario": "Norway Scenario"}, {"value": "0.0", "module": "A4", "scenario": "Sweden Scenario"}, {"value": "0.0", "module": "C1", "scenario": "Standard Scenario"}, {"value": "0.0", "module": "C2", "scenario": "Standard Scenario"}, {"value": "0.0", "module": "C3", "scenario": "Standard Scenario"}, {"value": "0.0", "module": "C4", "scenario": "Standard Scenario"}, {"value": "28.7", "module": "D", "scenario": "Standard Scenario"}, {"name": "referenceToUnitGroupDataSet", "value": {"shortDescription": [{"value": "MJ", "lang": "en"}], "type": "unit group data set", "refObjectId": "93a60a57-a3c8-11da-a746-0800200c9a66", "version": "03.00.000", "uri": "../unitgroups/93a60a57-a3c8-11da-a746-0800200c9a66.xml"}}]}, "flowProperties": [], "typeOfFlow": "Other flow", "classification": {"classHierarchy": "Größen / Umweltliche Größen / EPD EN 15804 / LCI Indikatoren", "name": "GaBiCategories"}}, {"dataSetInternalID": 4, "referenceToFlowDataSet": {"shortDescription": [{"value": "Exported thermal energy (EET)", "lang": "en"}, {"value": "Exportierte thermische Energie (EET)", "lang": "de"}, {"value": "Energía exportada termal (EET)", "lang": "es"}], "type": "flow data set", "refObjectId": "98daf38a-7a79-46d3-9a37-2b7bd0955810", "version": "30.00.000", "uri": "../flows/98daf38a-7a79-46d3-9a37-2b7bd0955810.xml"}, "exchange direction": "OUTPUT", "meanAmount": 0.0, "other": {"anies": [{"value": "0.0", "module": "A1", "scenario": "Standard Scenario"}, {"value": "0.0", "module": "A2", "scenario": "Standard Scenario"}, {"value": "0.0", "module": "A3", "scenario": "Standard Scenario"}, {"value": "0.0", "module": "A4", "scenario": "Norway Scenario"}, {"value": "0.0", "module": "A4", "scenario": "Sweden Scenario"}, {"value": "0.0", "module": "C1", "scenario": "Standard Scenario"}, {"value": "0.0", "module": "C2", "scenario": "Standard Scenario"}, {"value": "0.0", "module": "C3", "scenario": "Standard Scenario"}, {"value": "0.0", "module": "C4", "scenario": "Standard Scenario"}, {"value": "49.5", "module": "D", "scenario": "Standard Scenario"}, {"name": "referenceToUnitGroupDataSet", "value": {"shortDescription": [{"value": "MJ", "lang": "en"}], "type": "unit group data set", "refObjectId": "93a60a57-a3c8-11da-a746-0800200c9a66", "version": "03.00.000", "uri": "../unitgroups/93a60a57-a3c8-11da-a746-0800200c9a66.xml"}}]}, "flowProperties": [], "typeOfFlow": "Other flow", "classification": {"classHierarchy": "Größen / Umweltliche Größen / EPD EN 15804 / LCI Indikatoren", "name": "GaBiCategories"}}, {"dataSetInternalID": 5, "referenceToFlowDataSet": {"shortDescription": [{"value": "Use of net fresh water (FW)", "lang": "en"}, {"value": "Einsatz von Süßwasserressourcen (FW)", "lang": "de"}, {"value": "Uso neto de recursos de agua dulce (FW)", "lang": "es"}], "type": "flow data set", "refObjectId": "3cf952c8-f3a4-461d-8c96-96456ca62246", "version": "30.00.000", "uri": "../flows/3cf952c8-f3a4-461d-8c96-96456ca62246.xml"}, "exchange direction": "INPUT", "meanAmount": 0.0, "other": {"anies": [{"value": "21.3", "module": "A1", "scenario": "Standard Scenario"}, {"value": "0.538", "module": "A2", "scenario": "Standard Scenario"}, {"value": "2.44", "module": "A3", "scenario": "Standard Scenario"}, {"value": "0.2", "module": "A4", "scenario": "Norway Scenario"}, {"value": "0.0687", "module": "A4", "scenario": "Sweden Scenario"}, {"value": "0.00256", "module": "C1", "scenario": "Standard Scenario"}, {"value": "0.0119", "module": "C2", "scenario": "Standard Scenario"}, {"value": "0.0641", "module": "C3", "scenario": "Standard Scenario"}, {"value": "0.00157", "module": "C4", "scenario": "Standard Scenario"}, {"value": "-1.73", "module": "D", "scenario": "Standard Scenario"}, {"name": "referenceToUnitGroupDataSet", "value": {"shortDescription": [{"value": "m3", "lang": "en"}], "type": "unit group data set", "refObjectId": "cd950537-0a98-4044-9ba7-9f9a68d0a504", "version": "30.00.000", "uri": "../unitgroups/cd950537-0a98-4044-9ba7-9f9a68d0a504.xml"}}]}, "flowProperties": [], "typeOfFlow": "Other flow", "classification": {"classHierarchy": "Größen / Umweltliche Größen / EPD EN 15804 / LCI Indikatoren", "name": "GaBiCategories"}}, {"dataSetInternalID": 6, "referenceToFlowDataSet": {"shortDescription": [{"value": "Hazardous waste disposed (HWD)", "lang": "en"}, {"value": "Gefährlicher Abfall zur Deponie (HWD)", "lang": "de"}, {"value": "Residuos peligrosos eliminados (HWD)", "lang": "es"}], "type": "flow data set", "refObjectId": "430f9e0f-59b2-46a0-8e0d-55e0e84948fc", "version": "30.00.000", "uri": "../flows/430f9e0f-59b2-46a0-8e0d-55e0e84948fc.xml"}, "exchange direction": "OUTPUT", "meanAmount": 0.0, "other": {"anies": [{"value": "0.0788", "module": "A1", "scenario": "Standard Scenario"}, {"value": "0.0134", "module": "A2", "scenario": "Standard Scenario"}, {"value": "0.00549", "module": "A3", "scenario": "Standard Scenario"}, {"value": "0.00488", "module": "A4", "scenario": "Norway Scenario"}, {"value": "0.00167", "module": "A4", "scenario": "Sweden Scenario"}, {"value": "1.35E-4", "module": "C1", "scenario": "Standard Scenario"}, {"value": "2.48E-4", "module": "C2", "scenario": "Standard Scenario"}, {"value": "0.00204", "module": "C3", "scenario": "Standard Scenario"}, {"value": "2.2E-6", "module": "C4", "scenario": "Standard Scenario"}, {"value": "-0.0582", "module": "D", "scenario": "Standard Scenario"}, {"name": "referenceToUnitGroupDataSet", "value": {"shortDescription": [{"value": "kg", "lang": "en"}], "type": "unit group data set", "refObjectId": "ad38d542-3fe9-439d-9b95-2f5f7752acaf", "version": "30.00.000", "uri": "../unitgroups/ad38d542-3fe9-439d-9b95-2f5f7752acaf.xml"}}]}, "flowProperties": [], "typeOfFlow": "Other flow", "classification": {"classHierarchy": "Größen / Umweltliche Größen / EPD EN 15804 / LCI Indikatoren", "name": "GaBiCategories"}}, {"dataSetInternalID": 7, "referenceToFlowDataSet": {"shortDescription": [{"value": "Materials for energy recovery (MER)", "lang": "en"}, {"value": "Stoffe für die Energierückgewinnung (MER)", "lang": "de"}, {"value": "Materiales para valorización energética (recuperación de energía) (MER)", "lang": "es"}], "type": "flow data set", "refObjectId": "59a9181c-3aaf-46ee-8b13-2b3723b6e447", "version": "30.00.000", "uri": "../flows/59a9181c-3aaf-46ee-8b13-2b3723b6e447.xml"}, "exchange direction": "OUTPUT", "meanAmount": 0.0, "other": {"anies": [{"value": "0.0", "module": "A1", "scenario": "Standard Scenario"}, {"value": "0.0", "module": "A2", "scenario": "Standard Scenario"}, {"value": "0.0", "module": "A3", "scenario": "Standard Scenario"}, {"value": "0.0", "module": "A4", "scenario": "Norway Scenario"}, {"value": "0.0", "module": "A4", "scenario": "Sweden Scenario"}, {"value": "0.0", "module": "C1", "scenario": "Standard Scenario"}, {"value": "0.0", "module": "C2", "scenario": "Standard Scenario"}, {"value": "0.0", "module": "C3", "scenario": "Standard Scenario"}, {"value": "0.0", "module": "C4", "scenario": "Standard Scenario"}, {"value": "0.0", "module": "D", "scenario": "Standard Scenario"}, {"name": "referenceToUnitGroupDataSet", "value": {"shortDescription": [{"value": "kg", "lang": "en"}], "type": "unit group data set", "refObjectId": "ad38d542-3fe9-439d-9b95-2f5f7752acaf", "version": "30.00.000", "uri": "../unitgroups/ad38d542-3fe9-439d-9b95-2f5f7752acaf.xml"}}]}, "flowProperties": [], "typeOfFlow": "Other flow", "classification": {"classHierarchy": "Größen / Umweltliche Größen / EPD EN 15804 / LCI Indikatoren", "name": "GaBiCategories"}}, {"dataSetInternalID": 8, "referenceToFlowDataSet": {"shortDescription": [{"value": "Materials for recycling (MFR)", "lang": "en"}, {"value": "Stoffe zum Recycling (MFR)", "lang": "de"}, {"value": "Materiales para el reciclaje (MFR)", "lang": "es"}], "type": "flow data set", "refObjectId": "d7fe48a5-4103-49c8-9aae-b0b5dfdbd6ae", "version": "30.00.000", "uri": "../flows/d7fe48a5-4103-49c8-9aae-b0b5dfdbd6ae.xml"}, "exchange direction": "OUTPUT", "meanAmount": 0.0, "other": {"anies": [{"value": "0.0", "module": "A1", "scenario": "Standard Scenario"}, {"value": "0.0", "module": "A2", "scenario": "Standard Scenario"}, {"value": "81.2", "module": "A3", "scenario": "Standard Scenario"}, {"value": "0.0", "module": "A4", "scenario": "Norway Scenario"}, {"value": "0.0", "module": "A4", "scenario": "Sweden Scenario"}, {"value": "0.0", "module": "C1", "scenario": "Standard Scenario"}, {"value": "0.0", "module": "C2", "scenario": "Standard Scenario"}, {"value": "0.0", "module": "C3", "scenario": "Standard Scenario"}, {"value": "0.0", "module": "C4", "scenario": "Standard Scenario"}, {"value": "0.0", "module": "D", "scenario": "Standard Scenario"}, {"name": "referenceToUnitGroupDataSet", "value": {"shortDescription": [{"value": "kg", "lang": "en"}], "type": "unit group data set", "refObjectId": "ad38d542-3fe9-439d-9b95-2f5f7752acaf", "version": "30.00.000", "uri": "../unitgroups/ad38d542-3fe9-439d-9b95-2f5f7752acaf.xml"}}]}, "flowProperties": [], "typeOfFlow": "Other flow", "classification": {"classHierarchy": "Größen / Umweltliche Größen / EPD EN 15804 / LCI Indikatoren", "name": "GaBiCategories"}}, {"dataSetInternalID": 9, "referenceToFlowDataSet": {"shortDescription": [{"value": "Non-hazardous waste disposed (NHWD)", "lang": "en"}, {"value": "Entsorgter nicht gefährlicher Abfall (NHWD)", "lang": "de"}, {"value": "Residuos no peligrosos eliminados (NHWD)", "lang": "es"}], "type": "flow data set", "refObjectId": "b29ef66b-e286-4afa-949f-62f1a7b4d7fa", "version": "30.00.000", "uri": "../flows/b29ef66b-e286-4afa-949f-62f1a7b4d7fa.xml"}, "exchange direction": "OUTPUT", "meanAmount": 0.0, "other": {"anies": [{"value": "594.0", "module": "A1", "scenario": "Standard Scenario"}, {"value": "244.0", "module": "A2", "scenario": "Standard Scenario"}, {"value": "75.4", "module": "A3", "scenario": "Standard Scenario"}, {"value": "90.1", "module": "A4", "scenario": "Norway Scenario"}, {"value": "30.5", "module": "A4", "scenario": "Sweden Scenario"}, {"value": "0.0588", "module": "C1", "scenario": "Standard Scenario"}, {"value": "6.2", "module": "C2", "scenario": "Standard Scenario"}, {"value": "0.99", "module": "C3", "scenario": "Standard Scenario"}, {"value": "10.0", "module": "C4", "scenario": "Standard Scenario"}, {"value": "-46.5", "module": "D", "scenario": "Standard Scenario"}, {"name": "referenceToUnitGroupDataSet", "value": {"shortDescription": [{"value": "kg", "lang": "en"}], "type": "unit group data set", "refObjectId": "ad38d542-3fe9-439d-9b95-2f5f7752acaf", "version": "30.00.000", "uri": "../unitgroups/ad38d542-3fe9-439d-9b95-2f5f7752acaf.xml"}}]}, "flowProperties": [], "typeOfFlow": "Other flow", "classification": {"classHierarchy": "Größen / Umweltliche Größen / EPD EN 15804 / LCI Indikatoren", "name": "GaBiCategories"}}, {"dataSetInternalID": 10, "referenceToFlowDataSet": {"shortDescription": [{"value": "Use of non renewable secondary fuels (NRSF)", "lang": "en"}, {"value": "Nicht erneuerbare Sekundärbrennstoffe (NRSF)", "lang": "de"}, {"value": "Uso de combustibles secundarios no renovables (NRSF)", "lang": "es"}], "type": "flow data set", "refObjectId": "89def144-d39a-4287-b86f-efde453ddcb2", "version": "30.00.000", "uri": "../flows/89def144-d39a-4287-b86f-efde453ddcb2.xml"}, "exchange direction": "INPUT", "meanAmount": 0.0, "other": {"anies": [{"value": "0.0", "module": "A1", "scenario": "Standard Scenario"}, {"value": "0.0", "module": "A2", "scenario": "Standard Scenario"}, {"value": "0.0", "module": "A3", "scenario": "Standard Scenario"}, {"value": "0.0", "module": "A4", "scenario": "Norway Scenario"}, {"value": "0.0", "module": "A4", "scenario": "Sweden Scenario"}, {"value": "0.0", "module": "C1", "scenario": "Standard Scenario"}, {"value": "0.0", "module": "C2", "scenario": "Standard Scenario"}, {"value": "0.0", "module": "C3", "scenario": "Standard Scenario"}, {"value": "0.0", "module": "C4", "scenario": "Standard Scenario"}, {"value": "0.0", "module": "D", "scenario": "Standard Scenario"}, {"name": "referenceToUnitGroupDataSet", "value": {"shortDescription": [{"value": "MJ", "lang": "en"}], "type": "unit group data set", "refObjectId": "93a60a57-a3c8-11da-a746-0800200c9a66", "version": "03.00.000", "uri": "../unitgroups/93a60a57-a3c8-11da-a746-0800200c9a66.xml"}}]}, "flowProperties": [], "typeOfFlow": "Other flow", "classification": {"classHierarchy": "Größen / Umweltliche Größen / EPD EN 15804 / LCI Indikatoren", "name": "GaBiCategories"}}, {"dataSetInternalID": 11, "referenceToFlowDataSet": {"shortDescription": [{"value": "Use of non renewable primary energy (PENRE)", "lang": "en"}, {"value": "Nicht-erneuerbare Primärenergie als Energieträger (PENRE)", "lang": "de"}, {"value": "Uso de energía primaria no renovable, excluyendo los recursos de energía primaria no renovable utilizada como materia prima (PENRE)", "lang": "es"}], "type": "flow data set", "refObjectId": "ac857178-2b45-46ec-892a-a9a4332f0372", "version": "38.00.000", "uri": "../flows/ac857178-2b45-46ec-892a-a9a4332f0372.xml"}, "exchange direction": "INPUT", "meanAmount": 0.0, "other": {"anies": [{"value": "21400.0", "module": "A1", "scenario": "Standard Scenario"}, {"value": "5420.0", "module": "A2", "scenario": "Standard Scenario"}, {"value": "4220.0", "module": "A3", "scenario": "Standard Scenario"}, {"value": "2000.0", "module": "A4", "scenario": "Norway Scenario"}, {"value": "701.0", "module": "A4", "scenario": "Sweden Scenario"}, {"value": "52.7", "module": "C1", "scenario": "Standard Scenario"}, {"value": "104.0", "module": "C2", "scenario": "Standard Scenario"}, {"value": "821.0", "module": "C3", "scenario": "Standard Scenario"}, {"value": "1.56", "module": "C4", "scenario": "Standard Scenario"}, {"value": "-3660.0", "module": "D", "scenario": "Standard Scenario"}, {"name": "referenceToUnitGroupDataSet", "value": {"shortDescription": [{"value": "MJ", "lang": "en"}], "type": "unit group data set", "refObjectId": "93a60a57-a3c8-11da-a746-0800200c9a66", "version": "03.00.000", "uri": "../unitgroups/93a60a57-a3c8-11da-a746-0800200c9a66.xml"}}]}, "flowProperties": [], "typeOfFlow": "Other flow", "classification": {"classHierarchy": "Quantities", "name": "GaBiCategories"}}, {"dataSetInternalID": 12, "referenceToFlowDataSet": {"shortDescription": [{"value": "Use of non renewable primary energy resources used as raw materials (PENRM)", "lang": "en"}, {"value": "Nicht-erneuerbare Primärenergie zur stofflichen Nutzung (PENRM)", "lang": "de"}, {"value": "Uso de la energía primaria no renovable utilizada como materia prima (PENRM)", "lang": "es"}], "type": "flow data set", "refObjectId": "1421caa0-679d-4bf4-b282-0eb850ccae27", "version": "38.00.000", "uri": "../flows/1421caa0-679d-4bf4-b282-0eb850ccae27.xml"}, "exchange direction": "INPUT", "meanAmount": 0.0, "other": {"anies": [{"value": "9.24", "module": "A1", "scenario": "Standard Scenario"}, {"value": "0.0", "module": "A2", "scenario": "Standard Scenario"}, {"value": "4.7", "module": "A3", "scenario": "Standard Scenario"}, {"value": "0.0", "module": "A4", "scenario": "Norway Scenario"}, {"value": "0.0", "module": "A4", "scenario": "Sweden Scenario"}, {"value": "0.0", "module": "C1", "scenario": "Standard Scenario"}, {"value": "0.0", "module": "C2", "scenario": "Standard Scenario"}, {"value": "0.0", "module": "C3", "scenario": "Standard Scenario"}, {"value": "0.0", "module": "C4", "scenario": "Standard Scenario"}, {"value": "0.0", "module": "D", "scenario": "Standard Scenario"}, {"name": "referenceToUnitGroupDataSet", "value": {"shortDescription": [{"value": "MJ", "lang": "en"}], "type": "unit group data set", "refObjectId": "93a60a57-a3c8-11da-a746-0800200c9a66", "version": "03.00.000", "uri": "../unitgroups/93a60a57-a3c8-11da-a746-0800200c9a66.xml"}}]}, "flowProperties": [], "typeOfFlow": "Other flow", "classification": {"classHierarchy": "Quantities", "name": "GaBiCategories"}}, {"dataSetInternalID": 13, "referenceToFlowDataSet": {"shortDescription": [{"value": "Total use of non-renewable primary energy resources (PENRT)", "lang": "en"}, {"value": "Total nicht erneuerbare Primärenergie (PENRT)", "lang": "de"}, {"value": "Uso total de la energía primaria no renovable (energía primaria y recursos de energía primaria renovable utilizada como materia prima) (PENRT)", "lang": "es"}], "type": "flow data set", "refObjectId": "06159210-646b-4c8d-8583-da9b3b95a6c1", "version": "30.00.000", "uri": "../flows/06159210-646b-4c8d-8583-da9b3b95a6c1.xml"}, "exchange direction": "INPUT", "meanAmount": 0.0, "other": {"anies": [{"value": "21400.0", "module": "A1", "scenario": "Standard Scenario"}, {"value": "5420.0", "module": "A2", "scenario": "Standard Scenario"}, {"value": "4220.0", "module": "A3", "scenario": "Standard Scenario"}, {"value": "2000.0", "module": "A4", "scenario": "Norway Scenario"}, {"value": "701.0", "module": "A4", "scenario": "Sweden Scenario"}, {"value": "52.7", "module": "C1", "scenario": "Standard Scenario"}, {"value": "104.0", "module": "C2", "scenario": "Standard Scenario"}, {"value": "821.0", "module": "C3", "scenario": "Standard Scenario"}, {"value": "1.56", "module": "C4", "scenario": "Standard Scenario"}, {"value": "-3660.0", "module": "D", "scenario": "Standard Scenario"}, {"name": "referenceToUnitGroupDataSet", "value": {"shortDescription": [{"value": "MJ", "lang": "en"}], "type": "unit group data set", "refObjectId": "93a60a57-a3c8-11da-a746-0800200c9a66", "version": "03.00.000", "uri": "../unitgroups/93a60a57-a3c8-11da-a746-0800200c9a66.xml"}}]}, "flowProperties": [], "typeOfFlow": "Other flow", "classification": {"classHierarchy": "Größen / Umweltliche Größen / EPD EN 15804 / LCI Indikatoren", "name": "GaBiCategories"}}, {"dataSetInternalID": 14, "referenceToFlowDataSet": {"shortDescription": [{"value": "Use of renewable primary energy (PERE)", "lang": "en"}, {"value": "Erneuerbare Primärenergie als Energieträger (PERE)", "lang": "de"}, {"value": "Uso de energía primaria renovable excluyendo los recursos de energía primaria renovable utilizada como materia prima (PERE)", "lang": "es"}], "type": "flow data set", "refObjectId": "20f32be5-0398-4288-9b6d-accddd195317", "version": "38.00.000", "uri": "../flows/20f32be5-0398-4288-9b6d-accddd195317.xml"}, "exchange direction": "INPUT", "meanAmount": 0.0, "other": {"anies": [{"value": "2100.0", "module": "A1", "scenario": "Standard Scenario"}, {"value": "72.0", "module": "A2", "scenario": "Standard Scenario"}, {"value": "812.0", "module": "A3", "scenario": "Standard Scenario"}, {"value": "26.7", "module": "A4", "scenario": "Norway Scenario"}, {"value": "9.19", "module": "A4", "scenario": "Sweden Scenario"}, {"value": "0.268", "module": "C1", "scenario": "Standard Scenario"}, {"value": "1.22", "module": "C2", "scenario": "Standard Scenario"}, {"value": "9.86", "module": "C3", "scenario": "Standard Scenario"}, {"value": "0.0119", "module": "C4", "scenario": "Standard Scenario"}, {"value": "-90.2", "module": "D", "scenario": "Standard Scenario"}, {"name": "referenceToUnitGroupDataSet", "value": {"shortDescription": [{"value": "MJ", "lang": "en"}], "type": "unit group data set", "refObjectId": "93a60a57-a3c8-11da-a746-0800200c9a66", "version": "03.00.000", "uri": "../unitgroups/93a60a57-a3c8-11da-a746-0800200c9a66.xml"}}]}, "flowProperties": [], "typeOfFlow": "Other flow", "classification": {"classHierarchy": "Quantities", "name": "GaBiCategories"}}, {"dataSetInternalID": 15, "referenceToFlowDataSet": {"shortDescription": [{"value": "Use of renewable primary energy resources used as raw materials (PERM)", "lang": "en"}, {"value": "Erneuerbare Primärenergie zur stofflichen Nutzung (PERM)", "lang": "de"}, {"value": "Uso de energía primaria renovable utilizada como materia prima (PERM)", "lang": "es"}], "type": "flow data set", "refObjectId": "fb3ec0de-548d-4508-aea5-00b73bf6f702", "version": "38.00.000", "uri": "../flows/fb3ec0de-548d-4508-aea5-00b73bf6f702.xml"}, "exchange direction": "INPUT", "meanAmount": 0.0, "other": {"anies": [{"value": "0.0", "module": "A1", "scenario": "Standard Scenario"}, {"value": "0.0", "module": "A2", "scenario": "Standard Scenario"}, {"value": "181.0", "module": "A3", "scenario": "Standard Scenario"}, {"value": "0.0", "module": "A4", "scenario": "Norway Scenario"}, {"value": "0.0", "module": "A4", "scenario": "Sweden Scenario"}, {"value": "0.0", "module": "C1", "scenario": "Standard Scenario"}, {"value": "0.0", "module": "C2", "scenario": "Standard Scenario"}, {"value": "0.0", "module": "C3", "scenario": "Standard Scenario"}, {"value": "0.0", "module": "C4", "scenario": "Standard Scenario"}, {"value": "0.0", "module": "D", "scenario": "Standard Scenario"}, {"name": "referenceToUnitGroupDataSet", "value": {"shortDescription": [{"value": "MJ", "lang": "en"}], "type": "unit group data set", "refObjectId": "93a60a57-a3c8-11da-a746-0800200c9a66", "version": "03.00.000", "uri": "../unitgroups/93a60a57-a3c8-11da-a746-0800200c9a66.xml"}}]}, "flowProperties": [], "typeOfFlow": "Other flow", "classification": {"classHierarchy": "Quantities", "name": "GaBiCategories"}}, {"dataSetInternalID": 16, "referenceToFlowDataSet": {"shortDescription": [{"value": "Total use of renewable primary energy resources (PERT)", "lang": "en"}, {"value": "Total erneuerbare Primärenergie (PERT)", "lang": "de"}, {"value": "Uso total de la energía primaria renovable (energía primaria y recursos de energía primaria renovable utilizada como materia prima) (PERT)", "lang": "es"}], "type": "flow data set", "refObjectId": "53f97275-fa8a-4cdd-9024-65936002acd0", "version": "30.00.000", "uri": "../flows/53f97275-fa8a-4cdd-9024-65936002acd0.xml"}, "exchange direction": "INPUT", "meanAmount": 0.0, "other": {"anies": [{"value": "2100.0", "module": "A1", "scenario": "Standard Scenario"}, {"value": "72.0", "module": "A2", "scenario": "Standard Scenario"}, {"value": "994.0", "module": "A3", "scenario": "Standard Scenario"}, {"value": "26.7", "module": "A4", "scenario": "Norway Scenario"}, {"value": "9.19", "module": "A4", "scenario": "Sweden Scenario"}, {"value": "0.268", "module": "C1", "scenario": "Standard Scenario"}, {"value": "1.22", "module": "C2", "scenario": "Standard Scenario"}, {"value": "9.86", "module": "C3", "scenario": "Standard Scenario"}, {"value": "0.0119", "module": "C4", "scenario": "Standard Scenario"}, {"value": "-90.2", "module": "D", "scenario": "Standard Scenario"}, {"name": "referenceToUnitGroupDataSet", "value": {"shortDescription": [{"value": "MJ", "lang": "en"}], "type": "unit group data set", "refObjectId": "93a60a57-a3c8-11da-a746-0800200c9a66", "version": "03.00.000", "uri": "../unitgroups/93a60a57-a3c8-11da-a746-0800200c9a66.xml"}}]}, "flowProperties": [], "typeOfFlow": "Other flow", "classification": {"classHierarchy": "Größen / Umweltliche Größen / EPD EN 15804 / LCI Indikatoren", "name": "GaBiCategories"}}, {"dataSetInternalID": 17, "referenceToFlowDataSet": {"shortDescription": [{"value": "Use of renewable secondary fuels (RSF)", "lang": "en"}, {"value": "Erneuerbare Sekundärbrennstoffe (RSF)", "lang": "de"}, {"value": "Uso de combustibles secundarios renovables (RSF)", "lang": "es"}], "type": "flow data set", "refObjectId": "64333088-a55f-4aa2-9a31-c10b07816787", "version": "30.00.000", "uri": "../flows/64333088-a55f-4aa2-9a31-c10b07816787.xml"}, "exchange direction": "INPUT", "meanAmount": 0.0, "other": {"anies": [{"value": "0.0", "module": "A1", "scenario": "Standard Scenario"}, {"value": "0.0", "module": "A2", "scenario": "Standard Scenario"}, {"value": "0.0", "module": "A3", "scenario": "Standard Scenario"}, {"value": "0.0", "module": "A4", "scenario": "Norway Scenario"}, {"value": "0.0", "module": "A4", "scenario": "Sweden Scenario"}, {"value": "0.0", "module": "C1", "scenario": "Standard Scenario"}, {"value": "0.0", "module": "C2", "scenario": "Standard Scenario"}, {"value": "0.0", "module": "C3", "scenario": "Standard Scenario"}, {"value": "0.0", "module": "C4", "scenario": "Standard Scenario"}, {"value": "0.0", "module": "D", "scenario": "Standard Scenario"}, {"name": "referenceToUnitGroupDataSet", "value": {"shortDescription": [{"value": "MJ", "lang": "en"}], "type": "unit group data set", "refObjectId": "93a60a57-a3c8-11da-a746-0800200c9a66", "version": "03.00.000", "uri": "../unitgroups/93a60a57-a3c8-11da-a746-0800200c9a66.xml"}}]}, "flowProperties": [], "typeOfFlow": "Other flow", "classification": {"classHierarchy": "Größen / Umweltliche Größen / EPD EN 15804 / LCI Indikatoren", "name": "GaBiCategories"}}, {"dataSetInternalID": 18, "referenceToFlowDataSet": {"shortDescription": [{"value": "Radioactive waste disposed (RWD)", "lang": "en"}, {"value": "Entsorgter radioaktiver Abfall (RWD)", "lang": "de"}, {"value": "Residuos radiactivos eliminados (RWD)", "lang": "es"}], "type": "flow data set", "refObjectId": "3449546e-52ad-4b39-b809-9fb77cea8ff6", "version": "30.00.000", "uri": "../flows/3449546e-52ad-4b39-b809-9fb77cea8ff6.xml"}, "exchange direction": "OUTPUT", "meanAmount": 0.0, "other": {"anies": [{"value": "0.061", "module": "A1", "scenario": "Standard Scenario"}, {"value": "0.0348", "module": "A2", "scenario": "Standard Scenario"}, {"value": "0.0144", "module": "A3", "scenario": "Standard Scenario"}, {"value": "0.0129", "module": "A4", "scenario": "Norway Scenario"}, {"value": "0.0045", "module": "A4", "scenario": "Sweden Scenario"}, {"value": "3.45E-4", "module": "C1", "scenario": "Standard Scenario"}, {"value": "6.42E-4", "module": "C2", "scenario": "Standard Scenario"}, {"value": "0.00537", "module": "C3", "scenario": "Standard Scenario"}, {"value": "9.67E-6", "module": "C4", "scenario": "Standard Scenario"}, {"value": "0.00228", "module": "D", "scenario": "Standard Scenario"}, {"name": "referenceToUnitGroupDataSet", "value": {"shortDescription": [{"value": "kg", "lang": "en"}], "type": "unit group data set", "refObjectId": "ad38d542-3fe9-439d-9b95-2f5f7752acaf", "version": "30.00.000", "uri": "../unitgroups/ad38d542-3fe9-439d-9b95-2f5f7752acaf.xml"}}]}, "flowProperties": [], "typeOfFlow": "Other flow", "classification": {"classHierarchy": "Größen / Umweltliche Größen / EPD EN 15804 / LCI Indikatoren", "name": "GaBiCategories"}}, {"dataSetInternalID": 19, "referenceToFlowDataSet": {"shortDescription": [{"value": "Use of secondary material (SM)", "lang": "en"}, {"value": "Einsatz von Sekundärstoffen (SM)", "lang": "de"}, {"value": "Uso de materiales secundarios (SM)", "lang": "es"}], "type": "flow data set", "refObjectId": "c6a1f35f-2d09-4f54-8dfb-97e502e1ce92", "version": "30.00.000", "uri": "../flows/c6a1f35f-2d09-4f54-8dfb-97e502e1ce92.xml"}, "exchange direction": "INPUT", "meanAmount": 0.0, "other": {"anies": [{"value": "665.0", "module": "A1", "scenario": "Standard Scenario"}, {"value": "0.0", "module": "A2", "scenario": "Standard Scenario"}, {"value": "54.7", "module": "A3", "scenario": "Standard Scenario"}, {"value": "0.0", "module": "A4", "scenario": "Norway Scenario"}, {"value": "0.0", "module": "A4", "scenario": "Sweden Scenario"}, {"value": "0.0", "module": "C1", "scenario": "Standard Scenario"}, {"value": "0.0", "module": "C2", "scenario": "Standard Scenario"}, {"value": "940.0", "module": "C3", "scenario": "Standard Scenario"}, {"value": "0.0", "module": "C4", "scenario": "Standard Scenario"}, {"value": "0.018", "module": "D", "scenario": "Standard Scenario"}, {"name": "referenceToUnitGroupDataSet", "value": {"shortDescription": [{"value": "kg", "lang": "en"}], "type": "unit group data set", "refObjectId": "ad38d542-3fe9-439d-9b95-2f5f7752acaf", "version": "30.00.000", "uri": "../unitgroups/ad38d542-3fe9-439d-9b95-2f5f7752acaf.xml"}}]}, "flowProperties": [], "typeOfFlow": "Other flow", "classification": {"classHierarchy": "Größen / Umweltliche Größen / EPD EN 15804 / LCI Indikatoren", "name": "GaBiCategories"}}]}, "LCIAResults": {"LCIAResult": [{"referenceToLCIAMethodDataSet": {"shortDescription": [{"value": "Abiotic depletion potential - non-fossil resources (ADPE)", "lang": "en"}, {"value": "Potenzial für die Verknappung abiotischer Ressourcen – nicht fossile Ressourcen (ADPE)", "lang": "de"}], "type": "LCIA method data set", "refObjectId": "b2ad6494-c78d-11e6-9d9d-cec0c932ce01", "version": "01.00.011", "uri": "../lciamethods/b2ad6494-c78d-11e6-9d9d-cec0c932ce01.xml"}, "meanAmount": 0.0, "other": {"anies": [{"value": "0.0231", "module": "A1", "scenario": "Standard Scenario"}, {"value": "0.00916", "module": "A2", "scenario": "Standard Scenario"}, {"value": "0.00313", "module": "A3", "scenario": "Standard Scenario"}, {"value": "0.0034", "module": "A4", "scenario": "Norway Scenario"}, {"value": "0.00116", "module": "A4", "scenario": "Sweden Scenario"}, {"value": "5.53E-6", "module": "C1", "scenario": "Standard Scenario"}, {"value": "1.64E-4", "module": "C2", "scenario": "Standard Scenario"}, {"value": "9.41E-5", "module": "C3", "scenario": "Standard Scenario"}, {"value": "4.82E-7", "module": "C4", "scenario": "Standard Scenario"}, {"value": "-3.28E-4", "module": "D", "scenario": "Standard Scenario"}, {"name": "referenceToUnitGroupDataSet", "value": {"shortDescription": [{"value": "kg Sb-eq.", "lang": "en"}], "type": "unit group data set", "refObjectId": "54ccd2d9-a32a-4fc2-923d-f2c8c93e89d4", "version": "30.00.000", "uri": "../unitgroups/54ccd2d9-a32a-4fc2-923d-f2c8c93e89d4.xml"}}]}}, {"referenceToLCIAMethodDataSet": {"shortDescription": [{"value": "Abiotic depletion potential - fossil resources (ADPF)", "lang": "en"}, {"value": "Potenzial für die Verknappung abiotischer Ressourcen – fossile Brennstoffe (ADPF)", "lang": "de"}], "type": "LCIA method data set", "refObjectId": "b2ad6110-c78d-11e6-9d9d-cec0c932ce01", "version": "01.00.011", "uri": "../lciamethods/b2ad6110-c78d-11e6-9d9d-cec0c932ce01.xml"}, "meanAmount": 0.0, "other": {"anies": [{"value": "20100.0", "module": "A1", "scenario": "Standard Scenario"}, {"value": "5100.0", "module": "A2", "scenario": "Standard Scenario"}, {"value": "3910.0", "module": "A3", "scenario": "Standard Scenario"}, {"value": "1890.0", "module": "A4", "scenario": "Norway Scenario"}, {"value": "660.0", "module": "A4", "scenario": "Sweden Scenario"}, {"value": "49.6", "module": "C1", "scenario": "Standard Scenario"}, {"value": "97.7", "module": "C2", "scenario": "Standard Scenario"}, {"value": "774.0", "module": "C3", "scenario": "Standard Scenario"}, {"value": "1.47", "module": "C4", "scenario": "Standard Scenario"}, {"value": "-3520.0", "module": "D", "scenario": "Standard Scenario"}, {"name": "referenceToUnitGroupDataSet", "value": {"shortDescription": [{"value": "MJ", "lang": "en"}], "type": "unit group data set", "refObjectId": "93a60a57-a3c8-11da-a746-0800200c9a66", "version": "03.00.000", "uri": "../unitgroups/93a60a57-a3c8-11da-a746-0800200c9a66.xml"}}]}}, {"referenceToLCIAMethodDataSet": {"shortDescription": [{"value": "Acidification potential, Accumulated Exceedance (AP)", "lang": "en"}, {"value": "Versauerungspotenzial, kumulierte Überschreitung (AP)", "lang": "de"}], "type": "LCIA method data set", "refObjectId": "b5c611c6-def3-11e6-bf01-fe55135034f3", "version": "01.03.010", "uri": "../lciamethods/b5c611c6-def3-11e6-bf01-fe55135034f3.xml"}, "meanAmount": 0.0, "other": {"anies": [{"value": "8.01", "module": "A1", "scenario": "Standard Scenario"}, {"value": "1.38", "module": "A2", "scenario": "Standard Scenario"}, {"value": "1.15", "module": "A3", "scenario": "Standard Scenario"}, {"value": "0.44", "module": "A4", "scenario": "Norway Scenario"}, {"value": "0.207", "module": "A4", "scenario": "Sweden Scenario"}, {"value": "0.0377", "module": "C1", "scenario": "Standard Scenario"}, {"value": "0.0376", "module": "C2", "scenario": "Standard Scenario"}, {"value": "0.573", "module": "C3", "scenario": "Standard Scenario"}, {"value": "5.0E-4", "module": "C4", "scenario": "Standard Scenario"}, {"value": "-1.94", "module": "D", "scenario": "Standard Scenario"}, {"name": "referenceToUnitGroupDataSet", "value": {"shortDescription": [{"value": "mol H+-eq.", "lang": "en"}], "type": "unit group data set", "refObjectId": "42e089ac-92bf-4bf2-8ca1-5fc40d18f2ed", "version": "00.01.000", "uri": "../unitgroups/42e089ac-92bf-4bf2-8ca1-5fc40d18f2ed.xml"}}]}}, {"referenceToLCIAMethodDataSet": {"shortDescription": [{"value": "Eutrophication potential - freshwater (EP-freshwater)", "lang": "en"}, {"value": "Eutrophierungspotenzial - Süßwasser (EP-freshwater)", "lang": "de"}], "type": "LCIA method data set", "refObjectId": "b53ec18f-7377-4ad3-86eb-cc3f4f276b2b", "version": "01.00.011", "uri": "../lciamethods/b53ec18f-7377-4ad3-86eb-cc3f4f276b2b.xml"}, "meanAmount": 0.0, "other": {"anies": [{"value": "0.0972", "module": "A1", "scenario": "Standard Scenario"}, {"value": "0.00266", "module": "A2", "scenario": "Standard Scenario"}, {"value": "0.00956", "module": "A3", "scenario": "Standard Scenario"}, {"value": "9.89E-4", "module": "A4", "scenario": "Norway Scenario"}, {"value": "3.41E-4", "module": "A4", "scenario": "Sweden Scenario"}, {"value": "1.31E-5", "module": "C1", "scenario": "Standard Scenario"}, {"value": "6.53E-5", "module": "C2", "scenario": "Standard Scenario"}, {"value": "3.57E-4", "module": "C3", "scenario": "Standard Scenario"}, {"value": "5.9E-7", "module": "C4", "scenario": "Standard Scenario"}, {"value": "-0.0177", "module": "D", "scenario": "Standard Scenario"}, {"name": "referenceToUnitGroupDataSet", "value": {"shortDescription": [{"value": "kg P-eq.", "lang": "en"}], "type": "unit group data set", "refObjectId": "0429039d-a61d-4590-ba67-aa4a20a810a1", "version": "30.00.000", "uri": "../unitgroups/0429039d-a61d-4590-ba67-aa4a20a810a1.xml"}}]}}, {"referenceToLCIAMethodDataSet": {"shortDescription": [{"value": "Eutrophication potential - marine (EP-marine)", "lang": "en"}, {"value": "Eutrophierungspotenzial - Salzwasser (EP-marine)", "lang": "de"}], "type": "LCIA method data set", "refObjectId": "b5c619fa-def3-11e6-bf01-fe55135034f3", "version": "02.00.011", "uri": "../lciamethods/b5c619fa-def3-11e6-bf01-fe55135034f3.xml"}, "meanAmount": 0.0, "other": {"anies": [{"value": "1.7", "module": "A1", "scenario": "Standard Scenario"}, {"value": "0.41", "module": "A2", "scenario": "Standard Scenario"}, {"value": "0.264", "module": "A3", "scenario": "Standard Scenario"}, {"value": "0.0912", "module": "A4", "scenario": "Norway Scenario"}, {"value": "0.0451", "module": "A4", "scenario": "Sweden Scenario"}, {"value": "0.0167", "module": "C1", "scenario": "Standard Scenario"}, {"value": "0.0132", "module": "C2", "scenario": "Standard Scenario"}, {"value": "0.25", "module": "C3", "scenario": "Standard Scenario"}, {"value": "1.72E-4", "module": "C4", "scenario": "Standard Scenario"}, {"value": "-0.36", "module": "D", "scenario": "Standard Scenario"}, {"name": "referenceToUnitGroupDataSet", "value": {"shortDescription": [{"value": "kg N-eq.", "lang": "en"}], "type": "unit group data set", "refObjectId": "d05bb823-ecdf-4686-8c40-bf1d9257859f", "version": "00.00.003", "uri": "../unitgroups/d05bb823-ecdf-4686-8c40-bf1d9257859f.xml"}}]}}, {"referenceToLCIAMethodDataSet": {"shortDescription": [{"value": "Eutrophication potential - terrestrial (EP-terrestrial)", "lang": "en"}, {"value": "Eutrophierungspotenzial - Land (EP-terrestrial)", "lang": "de"}], "type": "LCIA method data set", "refObjectId": "b5c614d2-def3-11e6-bf01-fe55135034f3", "version": "01.02.010", "uri": "../lciamethods/b5c614d2-def3-11e6-bf01-fe55135034f3.xml"}, "meanAmount": 0.0, "other": {"anies": [{"value": "17.8", "module": "A1", "scenario": "Standard Scenario"}, {"value": "4.54", "module": "A2", "scenario": "Standard Scenario"}, {"value": "2.72", "module": "A3", "scenario": "Standard Scenario"}, {"value": "1.02", "module": "A4", "scenario": "Norway Scenario"}, {"value": "0.503", "module": "A4", "scenario": "Sweden Scenario"}, {"value": "0.183", "module": "C1", "scenario": "Standard Scenario"}, {"value": "0.146", "module": "C2", "scenario": "Standard Scenario"}, {"value": "2.75", "module": "C3", "scenario": "Standard Scenario"}, {"value": "0.0019", "module": "C4", "scenario": "Standard Scenario"}, {"value": "-4.24", "module": "D", "scenario": "Standard Scenario"}, {"name": "referenceToUnitGroupDataSet", "value": {"shortDescription": [{"value": "mol N-eq.", "lang": "en"}], "type": "unit group data set", "refObjectId": "71b4d617-0ec9-4d3f-b65e-e438940c2401", "version": "00.00.003", "uri": "../unitgroups/71b4d617-0ec9-4d3f-b65e-e438940c2401.xml"}}]}}, {"referenceToLCIAMethodDataSet": {"shortDescription": [{"value": "Potential Comparative Toxic Unit for ecosystems (ETP-fw)", "lang": "en"}, {"value": "Potenzielle Toxizitätsvergleichseinheit für Ökosysteme (ETP-fw)", "lang": "de"}], "type": "LCIA method data set", "refObjectId": "ee1082d1-b0f7-43ca-a1f0-21e2a4a74511", "version": "01.00.003", "uri": "../lciamethods/ee1082d1-b0f7-43ca-a1f0-21e2a4a74511.xml"}, "meanAmount": 0.0, "other": {"anies": [{"value": "58900.0", "module": "A1", "scenario": "Standard Scenario"}, {"value": "4090.0", "module": "A2", "scenario": "Standard Scenario"}, {"value": "4960.0", "module": "A3", "scenario": "Standard Scenario"}, {"value": "1510.0", "module": "A4", "scenario": "Norway Scenario"}, {"value": "526.0", "module": "A4", "scenario": "Sweden Scenario"}, {"value": "29.9", "module": "C1", "scenario": "Standard Scenario"}, {"value": "87.1", "module": "C2", "scenario": "Standard Scenario"}, {"value": "470.0", "module": "C3", "scenario": "Standard Scenario"}, {"value": "0.955", "module": "C4", "scenario": "Standard Scenario"}, {"value": "-16600.0", "module": "D", "scenario": "Standard Scenario"}, {"name": "referenceToUnitGroupDataSet", "value": {"shortDescription": [{"value": "CTUe", "lang": "en"}], "type": "unit group data set", "refObjectId": "aa959ded-f1eb-4efb-9c5c-2d60be36b3e6", "version": "00.00.003", "uri": "../unitgroups/aa959ded-f1eb-4efb-9c5c-2d60be36b3e6.xml"}}]}}, {"referenceToLCIAMethodDataSet": {"shortDescription": [{"value": "Global Warming Potential - biogenic (GWP-biogenic)", "lang": "en"}, {"value": "Globales Erwärmungspotenzial - biogen (GWP-biogenic)", "lang": "de"}], "type": "LCIA method data set", "refObjectId": "2356e1ab-0185-4db5-86e5-16de51c7485c", "version": "01.00.006", "uri": "../lciamethods/2356e1ab-0185-4db5-86e5-16de51c7485c.xml"}, "meanAmount": 0.0, "other": {"anies": [{"value": "-11.9", "module": "A1", "scenario": "Standard Scenario"}, {"value": "0.181", "module": "A2", "scenario": "Standard Scenario"}, {"value": "-22.5", "module": "A3", "scenario": "Standard Scenario"}, {"value": "0.065", "module": "A4", "scenario": "Norway Scenario"}, {"value": "0.0214", "module": "A4", "scenario": "Sweden Scenario"}, {"value": "0.001", "module": "C1", "scenario": "Standard Scenario"}, {"value": "0.00299", "module": "C2", "scenario": "Standard Scenario"}, {"value": "0.0598", "module": "C3", "scenario": "Standard Scenario"}, {"value": "1.04E-4", "module": "C4", "scenario": "Standard Scenario"}, {"value": "4.9", "module": "D", "scenario": "Standard Scenario"}, {"name": "referenceToUnitGroupDataSet", "value": {"shortDescription": [{"value": "kg CO2-eq.", "lang": "en"}], "type": "unit group data set", "refObjectId": "1ebf3012-d0db-4de2-aefd-ef30cedb0be1", "version": "30.00.000", "uri": "../unitgroups/1ebf3012-d0db-4de2-aefd-ef30cedb0be1.xml"}}]}}, {"referenceToLCIAMethodDataSet": {"shortDescription": [{"value": "Global Warming Potential - fossil fuels (GWP-fossil)", "lang": "en"}, {"value": "Globales Erwärmungspotenzial - fossil (GWP-fossil)", "lang": "de"}], "type": "LCIA method data set", "refObjectId": "5f635281-343e-44fb-83df-1971b155e6b6", "version": "01.00.009", "uri": "../lciamethods/5f635281-343e-44fb-83df-1971b155e6b6.xml"}, "meanAmount": 0.0, "other": {"anies": [{"value": "1590.0", "module": "A1", "scenario": "Standard Scenario"}, {"value": "338.0", "module": "A2", "scenario": "Standard Scenario"}, {"value": "251.0", "module": "A3", "scenario": "Standard Scenario"}, {"value": "125.0", "module": "A4", "scenario": "Norway Scenario"}, {"value": "44.1", "module": "A4", "scenario": "Sweden Scenario"}, {"value": "3.61", "module": "C1", "scenario": "Standard Scenario"}, {"value": "6.48", "module": "C2", "scenario": "Standard Scenario"}, {"value": "55.5", "module": "C3", "scenario": "Standard Scenario"}, {"value": "0.0527", "module": "C4", "scenario": "Standard Scenario"}, {"value": "-490.0", "module": "D", "scenario": "Standard Scenario"}, {"name": "referenceToUnitGroupDataSet", "value": {"shortDescription": [{"value": "kg CO2-eq.", "lang": "en"}], "type": "unit group data set", "refObjectId": "1ebf3012-d0db-4de2-aefd-ef30cedb0be1", "version": "30.00.000", "uri": "../unitgroups/1ebf3012-d0db-4de2-aefd-ef30cedb0be1.xml"}}]}}, {"referenceToLCIAMethodDataSet": {"shortDescription": [{"value": "Global Warming Potential - land use and land use change (GWP-luluc)", "lang": "en"}, {"value": "Globales Erwärmungspotenzial - luluc (GWP-luluc)", "lang": "de"}], "type": "LCIA method data set", "refObjectId": "4331bbdb-978a-490d-8707-eeb047f01a55", "version": "01.00.006", "uri": "../lciamethods/4331bbdb-978a-490d-8707-eeb047f01a55.xml"}, "meanAmount": 0.0, "other": {"anies": [{"value": "28.7", "module": "A1", "scenario": "Standard Scenario"}, {"value": "0.118", "module": "A2", "scenario": "Standard Scenario"}, {"value": "7.93", "module": "A3", "scenario": "Standard Scenario"}, {"value": "0.0454", "module": "A4", "scenario": "Norway Scenario"}, {"value": "0.0166", "module": "A4", "scenario": "Sweden Scenario"}, {"value": "2.84E-4", "module": "C1", "scenario": "Standard Scenario"}, {"value": "0.00237", "module": "C2", "scenario": "Standard Scenario"}, {"value": "0.00773", "module": "C3", "scenario": "Standard Scenario"}, {"value": "1.47E-5", "module": "C4", "scenario": "Standard Scenario"}, {"value": "0.326", "module": "D", "scenario": "Standard Scenario"}, {"name": "referenceToUnitGroupDataSet", "value": {"shortDescription": [{"value": "kg CO2-eq.", "lang": "en"}], "type": "unit group data set", "refObjectId": "1ebf3012-d0db-4de2-aefd-ef30cedb0be1", "version": "30.00.000", "uri": "../unitgroups/1ebf3012-d0db-4de2-aefd-ef30cedb0be1.xml"}}]}}, {"referenceToLCIAMethodDataSet": {"shortDescription": [{"value": "Global Warming Potential - total (GWP-total)", "lang": "en"}, {"value": "Globales Erwärmungspotenzial - total (GWP-total)", "lang": "de"}], "type": "LCIA method data set", "refObjectId": "6a37f984-a4b3-458a-a20a-64418c145fa2", "version": "04.00.017", "uri": "../lciamethods/6a37f984-a4b3-458a-a20a-64418c145fa2.xml"}, "meanAmount": 0.0, "other": {"anies": [{"value": "1600.0", "module": "A1", "scenario": "Standard Scenario"}, {"value": "339.0", "module": "A2", "scenario": "Standard Scenario"}, {"value": "237.0", "module": "A3", "scenario": "Standard Scenario"}, {"value": "125.0", "module": "A4", "scenario": "Norway Scenario"}, {"value": "44.1", "module": "A4", "scenario": "Sweden Scenario"}, {"value": "3.61", "module": "C1", "scenario": "Standard Scenario"}, {"value": "6.48", "module": "C2", "scenario": "Standard Scenario"}, {"value": "55.5", "module": "C3", "scenario": "Standard Scenario"}, {"value": "0.0528", "module": "C4", "scenario": "Standard Scenario"}, {"value": "-485.0", "module": "D", "scenario": "Standard Scenario"}, {"name": "referenceToUnitGroupDataSet", "value": {"shortDescription": [{"value": "kg CO2-eq.", "lang": "en"}], "type": "unit group data set", "refObjectId": "1ebf3012-d0db-4de2-aefd-ef30cedb0be1", "version": "30.00.000", "uri": "../unitgroups/1ebf3012-d0db-4de2-aefd-ef30cedb0be1.xml"}}]}}, {"referenceToLCIAMethodDataSet": {"shortDescription": [{"value": "Potential Comparative Toxic Unit for humans - cancer effects (HTP-c)", "lang": "en"}, {"value": "Potenzielle Toxizitätsvergleichseinheit für den Menschen - kanzerogene Wirkung (HTP-c)", "lang": "de"}], "type": "LCIA method data set", "refObjectId": "2299222a-bbd8-474f-9d4f-4dd1f18aea7c", "version": "01.00.004", "uri": "../lciamethods/2299222a-bbd8-474f-9d4f-4dd1f18aea7c.xml"}, "meanAmount": 0.0, "other": {"anies": [{"value": "1.42E-5", "module": "A1", "scenario": "Standard Scenario"}, {"value": "1.15E-7", "module": "A2", "scenario": "Standard Scenario"}, {"value": "1.25E-6", "module": "A3", "scenario": "Standard Scenario"}, {"value": "4.3E-8", "module": "A4", "scenario": "Norway Scenario"}, {"value": "1.56E-8", "module": "A4", "scenario": "Sweden Scenario"}, {"value": "1.05E-9", "module": "C1", "scenario": "Standard Scenario"}, {"value": "2.83E-9", "module": "C2", "scenario": "Standard Scenario"}, {"value": "1.64E-8", "module": "C3", "scenario": "Standard Scenario"}, {"value": "2.21E-11", "module": "C4", "scenario": "Standard Scenario"}, {"value": "-2.24E-7", "module": "D", "scenario": "Standard Scenario"}, {"name": "referenceToUnitGroupDataSet", "value": {"shortDescription": [{"value": "CTUh", "lang": "en"}], "type": "unit group data set", "refObjectId": "d4c9523e-2d7e-49fd-8469-998f547d3a70", "version": "00.00.003", "uri": "../unitgroups/d4c9523e-2d7e-49fd-8469-998f547d3a70.xml"}}]}}, {"referenceToLCIAMethodDataSet": {"shortDescription": [{"value": "Potential Comparative Toxic Unit for humans - non-cancer effects (HTP-nc)", "lang": "en"}, {"value": "Potenzielle Toxizitätsvergleichseinheit für den Menschen - nicht kanzerogene Wirkung (HTP-nc)", "lang": "de"}], "type": "LCIA method data set", "refObjectId": "3af763a5-b7a1-48c9-9cee-1f223481fcef", "version": "01.00.003", "uri": "../lciamethods/3af763a5-b7a1-48c9-9cee-1f223481fcef.xml"}, "meanAmount": 0.0, "other": {"anies": [{"value": "2.33E-4", "module": "A1", "scenario": "Standard Scenario"}, {"value": "4.46E-6", "module": "A2", "scenario": "Standard Scenario"}, {"value": "2.77E-5", "module": "A3", "scenario": "Standard Scenario"}, {"value": "1.59E-6", "module": "A4", "scenario": "Norway Scenario"}, {"value": "5.49E-7", "module": "A4", "scenario": "Sweden Scenario"}, {"value": "2.57E-8", "module": "C1", "scenario": "Standard Scenario"}, {"value": "9.53E-8", "module": "C2", "scenario": "Standard Scenario"}, {"value": "4.04E-7", "module": "C3", "scenario": "Standard Scenario"}, {"value": "6.79E-10", "module": "C4", "scenario": "Standard Scenario"}, {"value": "8.79E-5", "module": "D", "scenario": "Standard Scenario"}, {"name": "referenceToUnitGroupDataSet", "value": {"shortDescription": [{"value": "CTUh", "lang": "en"}], "type": "unit group data set", "refObjectId": "d4c9523e-2d7e-49fd-8469-998f547d3a70", "version": "00.00.003", "uri": "../unitgroups/d4c9523e-2d7e-49fd-8469-998f547d3a70.xml"}}]}}, {"referenceToLCIAMethodDataSet": {"shortDescription": [{"value": "Potential Human exposure efficiency relative to U235 (IRP)", "lang": "en"}, {"value": "Potenzielle Wirkung durch Exposition des Menschen mit U235 (IRP)", "lang": "de"}], "type": "LCIA method data set", "refObjectId": "b5c632be-def3-11e6-bf01-fe55135034f3", "version": "01.00.012", "uri": "../lciamethods/b5c632be-def3-11e6-bf01-fe55135034f3.xml"}, "meanAmount": 0.0, "other": {"anies": [{"value": "65.3", "module": "A1", "scenario": "Standard Scenario"}, {"value": "22.3", "module": "A2", "scenario": "Standard Scenario"}, {"value": "14.2", "module": "A3", "scenario": "Standard Scenario"}, {"value": "8.24", "module": "A4", "scenario": "Norway Scenario"}, {"value": "2.88", "module": "A4", "scenario": "Sweden Scenario"}, {"value": "0.213", "module": "C1", "scenario": "Standard Scenario"}, {"value": "0.409", "module": "C2", "scenario": "Standard Scenario"}, {"value": "3.45", "module": "C3", "scenario": "Standard Scenario"}, {"value": "0.00604", "module": "C4", "scenario": "Standard Scenario"}, {"value": "7.51", "module": "D", "scenario": "Standard Scenario"}, {"name": "referenceToUnitGroupDataSet", "value": {"shortDescription": [{"value": "kgBq U235-eq.", "lang": "en"}], "type": "unit group data set", "refObjectId": "456b05bf-1415-44a9-9993-02452f554c09", "version": "00.00.003", "uri": "../unitgroups/456b05bf-1415-44a9-9993-02452f554c09.xml"}}]}}, {"referenceToLCIAMethodDataSet": {"shortDescription": [{"value": "Depletion potential of the stratospheric ozone layer (ODP)", "lang": "en"}, {"value": "Abbaupotenzial der stratosphärischen Ozonschicht (ODP)", "lang": "de"}], "type": "LCIA method data set", "refObjectId": "b5c629d6-def3-11e6-bf01-fe55135034f3", "version": "02.00.013", "uri": "../lciamethods/b5c629d6-def3-11e6-bf01-fe55135034f3.xml"}, "meanAmount": 0.0, "other": {"anies": [{"value": "1.14E-4", "module": "A1", "scenario": "Standard Scenario"}, {"value": "7.69E-5", "module": "A2", "scenario": "Standard Scenario"}, {"value": "3.4E-5", "module": "A3", "scenario": "Standard Scenario"}, {"value": "2.84E-5", "module": "A4", "scenario": "Norway Scenario"}, {"value": "9.95E-6", "module": "A4", "scenario": "Sweden Scenario"}, {"value": "7.79E-7", "module": "C1", "scenario": "Standard Scenario"}, {"value": "1.43E-6", "module": "C2", "scenario": "Standard Scenario"}, {"value": "1.18E-5", "module": "C3", "scenario": "Standard Scenario"}, {"value": "2.17E-8", "module": "C4", "scenario": "Standard Scenario"}, {"value": "-1.28E-5", "module": "D", "scenario": "Standard Scenario"}, {"name": "referenceToUnitGroupDataSet", "value": {"shortDescription": [{"value": "kg CFC-11-eq.", "lang": "en"}], "type": "unit group data set", "refObjectId": "d9e957c9-7309-4474-bf3a-7777df6c4e5b", "version": "25.00.000", "uri": "../unitgroups/d9e957c9-7309-4474-bf3a-7777df6c4e5b.xml"}}]}}, {"referenceToLCIAMethodDataSet": {"shortDescription": [{"value": "Potential incidence of disease due to PM emissions (PM)", "lang": "en"}, {"value": "Potenzielles Auftreten von Krankheiten aufgrund von Feinstaubemissionen (PM)", "lang": "de"}], "type": "LCIA method data set", "refObjectId": "b5c602c6-def3-11e6-bf01-fe55135034f3", "version": "02.00.012", "uri": "../lciamethods/b5c602c6-def3-11e6-bf01-fe55135034f3.xml"}, "meanAmount": 0.0, "other": {"anies": [{"value": "1.42E-4", "module": "A1", "scenario": "Standard Scenario"}, {"value": "2.36E-5", "module": "A2", "scenario": "Standard Scenario"}, {"value": "1.69E-5", "module": "A3", "scenario": "Standard Scenario"}, {"value": "7.88E-6", "module": "A4", "scenario": "Norway Scenario"}, {"value": "2.72E-6", "module": "A4", "scenario": "Sweden Scenario"}, {"value": "1.0E-6", "module": "C1", "scenario": "Standard Scenario"}, {"value": "5.83E-7", "module": "C2", "scenario": "Standard Scenario"}, {"value": "1.5E-5", "module": "C3", "scenario": "Standard Scenario"}, {"value": "9.72E-9", "module": "C4", "scenario": "Standard Scenario"}, {"value": "-2.95E-5", "module": "D", "scenario": "Standard Scenario"}, {"name": "referenceToUnitGroupDataSet", "value": {"shortDescription": [{"value": "Disease incidence", "lang": "en"}], "type": "unit group data set", "refObjectId": "3883559b-648f-4afc-8ba2-0bd24f3affa3", "version": "00.00.003", "uri": "../unitgroups/3883559b-648f-4afc-8ba2-0bd24f3affa3.xml"}}]}}, {"referenceToLCIAMethodDataSet": {"shortDescription": [{"value": "Photochemical Ozone Creation Potential (POCP)", "lang": "en"}, {"value": "Bildungspotenzial für troposphärisches Ozon (POCP)", "lang": "de"}], "type": "LCIA method data set", "refObjectId": "b5c610fe-def3-11e6-bf01-fe55135034f3", "version": "02.00.015", "uri": "../lciamethods/b5c610fe-def3-11e6-bf01-fe55135034f3.xml"}, "meanAmount": 0.0, "other": {"anies": [{"value": "7.38", "module": "A1", "scenario": "Standard Scenario"}, {"value": "1.39", "module": "A2", "scenario": "Standard Scenario"}, {"value": "0.861", "module": "A3", "scenario": "Standard Scenario"}, {"value": "0.36", "module": "A4", "scenario": "Norway Scenario"}, {"value": "0.163", "module": "A4", "scenario": "Sweden Scenario"}, {"value": "0.0502", "module": "C1", "scenario": "Standard Scenario"}, {"value": "0.0417", "module": "C2", "scenario": "Standard Scenario"}, {"value": "0.755", "module": "C3", "scenario": "Standard Scenario"}, {"value": "5.51E-4", "module": "C4", "scenario": "Standard Scenario"}, {"value": "-2.79", "module": "D", "scenario": "Standard Scenario"}, {"name": "referenceToUnitGroupDataSet", "value": {"shortDescription": [{"value": "kg NMVOC-eq.", "lang": "en"}], "type": "unit group data set", "refObjectId": "d27c25f8-fbc1-44c6-b47b-4adbae4199c6", "version": "00.00.003", "uri": "../unitgroups/d27c25f8-fbc1-44c6-b47b-4adbae4199c6.xml"}}]}}, {"referenceToLCIAMethodDataSet": {"shortDescription": [{"value": "Potential Soil quality index (SQP)", "lang": "en"}, {"value": "Potenzieller Bodenqualitätsindex (SQP)", "lang": "de"}], "type": "LCIA method data set", "refObjectId": "b2ad6890-c78d-11e6-9d9d-cec0c932ce01", "version": "01.00.011", "uri": "../lciamethods/b2ad6890-c78d-11e6-9d9d-cec0c932ce01.xml"}, "meanAmount": 0.0, "other": {"anies": [{"value": "7780.0", "module": "A1", "scenario": "Standard Scenario"}, {"value": "3520.0", "module": "A2", "scenario": "Standard Scenario"}, {"value": "5130.0", "module": "A3", "scenario": "Standard Scenario"}, {"value": "1300.0", "module": "A4", "scenario": "Norway Scenario"}, {"value": "442.0", "module": "A4", "scenario": "Sweden Scenario"}, {"value": "6.33", "module": "C1", "scenario": "Standard Scenario"}, {"value": "84.7", "module": "C2", "scenario": "Standard Scenario"}, {"value": "116.0", "module": "C3", "scenario": "Standard Scenario"}, {"value": "3.09", "module": "C4", "scenario": "Standard Scenario"}, {"value": "-1630.0", "module": "D", "scenario": "Standard Scenario"}, {"name": "referenceToUnitGroupDataSet", "value": {"shortDescription": [{"value": "dimensionless", "lang": "en"}], "type": "unit group data set", "refObjectId": "f130951c-e67f-4f7f-8dd4-665de3974e18", "version": "00.00.004", "uri": "../unitgroups/f130951c-e67f-4f7f-8dd4-665de3974e18.xml"}}]}}, {"referenceToLCIAMethodDataSet": {"shortDescription": [{"value": "Water (user) deprivation potential (WDP)", "lang": "en"}, {"value": "Wasser-Entzugspotenzial (Benutzer) (WDP)", "lang": "de"}], "type": "LCIA method data set", "refObjectId": "b2ad66ce-c78d-11e6-9d9d-cec0c932ce01", "version": "03.00.015", "uri": "../lciamethods/b2ad66ce-c78d-11e6-9d9d-cec0c932ce01.xml"}, "meanAmount": 0.0, "other": {"anies": [{"value": "701.0", "module": "A1", "scenario": "Standard Scenario"}, {"value": "14.2", "module": "A2", "scenario": "Standard Scenario"}, {"value": "75.4", "module": "A3", "scenario": "Standard Scenario"}, {"value": "5.29", "module": "A4", "scenario": "Norway Scenario"}, {"value": "1.82", "module": "A4", "scenario": "Sweden Scenario"}, {"value": "0.0665", "module": "C1", "scenario": "Standard Scenario"}, {"value": "0.35", "module": "C2", "scenario": "Standard Scenario"}, {"value": "1.34", "module": "C3", "scenario": "Standard Scenario"}, {"value": "0.066", "module": "C4", "scenario": "Standard Scenario"}, {"value": "-90.0", "module": "D", "scenario": "Standard Scenario"}, {"name": "referenceToUnitGroupDataSet", "value": {"shortDescription": [{"value": "m3 world eq. deprived", "lang": "en"}], "type": "unit group data set", "refObjectId": "6ae2df01-888e-46c8-b17d-49fa3869b476", "version": "00.00.003", "uri": "../unitgroups/6ae2df01-888e-46c8-b17d-49fa3869b476.xml"}}]}}]}, "otherAttributes": {"{http://www.indata.network/EPD/2019}epd-version": "1.2"}, "version": "1.1"}