{"processInformation": {"dataSetInformation": {"UUID": "ba9c150e-4334-4bdf-ba93-337ea848c7ea", "name": {"baseName": [{"value": "ETICS gluing and coating silicate dispersion plaster", "lang": "en"}, {"value": "WDVS Verklebung und Beschichtung Silikat-Dispersionsputz", "lang": "de"}], "functionalUnitFlowProperties": [{"value": "12,3 kg/m2", "lang": "en"}]}, "classificationInformation": {"classification": [{"class": [{"value": "Dämmstoffe", "level": 0, "classId": "2"}, {"value": "Wärmedämmverbundsystem", "level": 1, "classId": "2.21"}, {"value": "Wärmedämmverbundsystem", "level": 2, "classId": "2.21.01"}], "name": "oekobau.dat"}]}, "generalComment": [{"value": "This data set has been modeled according to the European Standard EN 15804+A2 for Sustainable Building. Results are depicted in modules that allow the structured expression of results over the entire life cycle.", "lang": "en"}, {"value": "Dieser Datensatz wurde nach dem European Standard EN 15804+A2 für Nachhaltiges Bauen modelliert. Ergebnisse werden in Modulen abgebildet, die den strukturierten Ausdruck von Ergebnissen über den gesamten Lebenszyklus zulassen.", "lang": "de"}], "other": {"anies": [{"margins": 10, "description": [{"value": "Product system almost completely covered. Good technological, temporal and geographic representativeness.", "lang": "en"}, {"value": "Produktsystem weitgehend vollständig abgebildet. Gute technologische, zeitliche und geographische Repräsentativität.", "lang": "de"}]}]}}, "quantitativeReference": {"referenceToReferenceFlow": [100171], "type": "Reference flow(s)"}, "time": {"referenceYear": 2023, "dataSetValidUntil": 2026, "timeRepresentativenessDescription": [{"value": "Annual average", "lang": "en"}, {"value": "Jährlicher Durchschnitt", "lang": "de"}]}, "geography": {"locationOfOperationSupplyOrProduction": {"descriptionOfRestrictions": [{"value": "The data set represents the country specific situation in Germany, focusing on the main technologies, the region specific characteristics and / or import statistics.", "lang": "en"}, {"value": "Der Datensatz bildet die länderspezifische Situation in Deutschland ab. Dabei werden Haupttechnologien, spezifische regionale Charakteristiken und ggf. Importstatistiken berücksichtigt.", "lang": "de"}], "location": "DE"}}, "technology": {"technologyDescriptionAndIncludedProcesses": [{"value": "This dataset covers an external wall insulation system (EWIS) with silicone resin plaster. The insulation material and the wall material are not considered in this process. The system has the following structure:  \nReinforcement (mineral) 4.0 kg/m2   \nGlass fibre mesh 0.18 kg/m2 \nReinforcement (synthetic resin trowel) 4.0 kg/m2  \nPrecoat (synthetic resin)  0.3 kg/m2\nSilicone resin plaster 4.0 kg/m2\nThe system boundaries comprise the cradle to gate life cycle of the EWIS.\n\nIn the disposal phase, a manual dismantling (no loads) is assumed in module C1. The transport in module C2 to the landfill site takes place with a truck (50km). In C3, if relevant, a packaging with PE foil is taken into account (for example, for mineral fiber products. 0.0125 kg foil per kg of discarded material). In module C4 the average landfill emissions corresponding to the product (reference country Germany) are shown. The use of landfill gas is not taken into account.", "lang": "en"}, {"value": "Bei dem WDVS handelt es sich um ein Außenwand-Dämmsystem. Das Dämmmaterial und das Wandmaterial sind nicht im Prozess berücksichtigt. Das System weist folgende Spezifikationen auf: Außenwand-Dämmsystem Silikatdispersionsputz: Kleber (mineralisch) 4,0 kg/m2, Glasfasergewebe 0,18 kg/m2, Armierung (mineralisch) 4,0 kg/m2, Voranstrich (Silikatdispersion) 0,3 kg/m2, Silikatdispersionsputz 4,0 kg/m2. Dieser Datensatz umfasst die Lebenswegabschnitte cradle to gate, d.h. die Herstellung von Vorprodukten und Verpackungen ist  berücksichtigt. \n\nIn der Entsorgungsphase wird ein manueller Rückbau (lastenfrei) in Modul C1 angenommen. Der Transport in Modul C2 zur Deponie erfolgt mit einem LKW (50km). In C3 wird, sofern relevant, eine Verpackung mit PE-Folie berücksichtigt (z.B. bei Mineralfaserprodukten, 0,0125 kg Folie je kg entsorgtes Material). In Modul C4 werden dem Produkt entsprechende, durchschnittliche Deponieemissionen (Bezugsraum Deutschland) ausgewiesen. Die Nutzung von Deponiegas wird nicht berücksichtigt.", "lang": "de"}], "technologicalApplicability": [{"value": "This product can be used in construction.", "lang": "en"}, {"value": "Dieses Produkt kann im Baubereich verwendet werden.", "lang": "de"}], "referenceToTechnologyFlowDiagrammOrPicture": [{"shortDescription": [{"value": "construction_40_wdvs_engl.jpg", "lang": "en"}], "type": "source data set", "refObjectId": "a3903b69-efc1-47aa-9f76-56713bab8952", "version": "24.01.000", "uri": "../sources/a3903b69-efc1-47aa-9f76-56713bab8952.xml"}]}}, "modellingAndValidation": {"LCIMethodAndAllocation": {"typeOfDataSet": "EPD", "other": {"anies": [{"name": "subType", "value": "generic dataset"}]}}, "dataSourcesTreatmentAndRepresentativeness": {"referenceToDataSource": [{"shortDescription": [{"value": "Eco profiles of production systems for silicones, 2002", "lang": "en"}], "type": "source data set", "refObjectId": "235515b2-7bb4-11db-9fe1-0800200c9a66", "version": "24.01.000", "uri": "../sources/235515b2-7bb4-11db-9fe1-0800200c9a66.xml"}, {"shortDescription": [{"value": "Documentation of data quality management", "lang": "en"}], "type": "source data set", "refObjectId": "e3bd9bbf-2c3c-42aa-8892-fd13f1065ca5", "version": "24.01.000", "uri": "../sources/e3bd9bbf-2c3c-42aa-8892-fd13f1065ca5.xml"}, {"shortDescription": [{"value": "GaBi Database Edition 2021, CUP2021.01", "lang": "en"}], "type": "source data set", "refObjectId": "1cece811-7501-44d4-8067-9259bd5cb835", "version": "00.01.000", "uri": "../sources/1cece811-7501-44d4-8067-9259bd5cb835.xml"}, {"shortDescription": [{"value": "Sphera Managed LCA Content Databases (all versions)", "lang": "en"}], "type": "source data set", "refObjectId": "28d74cc0-db8b-4d7e-bc44-5f6d56ce0c4a", "version": "00.03.002", "uri": "../sources/28d74cc0-db8b-4d7e-bc44-5f6d56ce0c4a.xml"}], "useAdviceForDataSet": [{"value": "The data set represents a cradle to gate inventory. It can be used to characterise the supply chain situation of the respective commodity in a representative manner. Combination with individual unit processes using this commodity enables the generation of user-specific (product) LCAs.", "lang": "en"}, {"value": "Der Datensatz repräsentiert ein Cradle to Gate Inventar. Er kann verwendet werden, um die Lieferkette des jeweiligen Produktes in einer repräsentativen Weise zu charakterisieren. Die Kombination mit einzelnen Einheitenprozessen und diesem Produkt ermöglicht die Erstellung von anwenderspezifischen (Produkt-) LCAs.", "lang": "de"}]}, "validation": {"review": [{"referenceToNameOfReviewerAndInstitution": [{"shortDescription": [{"value": "Sphera Solutions GmbH", "lang": "en"}], "type": "contact data set", "refObjectId": "d7fa0337-f279-430d-becf-7f3111a85010", "version": "24.01.000", "uri": "../contacts/d7fa0337-f279-430d-becf-7f3111a85010.xml"}], "type": "Dependent internal review"}, {"referenceToNameOfReviewerAndInstitution": [{"shortDescription": [{"value": "Sphera Product Sustainability user forum", "lang": "en"}], "type": "contact data set", "refObjectId": "8f1306f0-7b83-4f36-a537-aa83f0498266", "version": "24.01.000", "uri": "../contacts/8f1306f0-7b83-4f36-a537-aa83f0498266.xml"}], "type": "Independent external review"}]}, "complianceDeclarations": {"compliance": [{"referenceToComplianceSystem": {"shortDescription": [{"value": "EN 15804+A2 (EF 3.1)", "lang": "de"}, {"value": "EN 15804+A2 (EF 3.1)", "lang": "en"}], "type": "source data set", "refObjectId": "d4aa3ec7-b1d7-4a4a-a6cb-37af88dcc902", "version": "00.01.000", "uri": "../sources/d4aa3ec7-b1d7-4a4a-a6cb-37af88dcc902.xml"}, "approvalOfOverallCompliance": "Fully compliant"}]}}, "administrativeInformation": {"dataGenerator": {"referenceToPersonOrEntityGeneratingTheDataSet": [{"shortDescription": [{"value": "Sphera Solutions GmbH", "lang": "en"}], "type": "contact data set", "refObjectId": "d7fa0337-f279-430d-becf-7f3111a85010", "version": "24.01.000", "uri": "../contacts/d7fa0337-f279-430d-becf-7f3111a85010.xml"}]}, "dataEntryBy": {"timeStamp": 1718121678000, "referenceToDataSetFormat": [{"shortDescription": [{"value": "ILCD format 1.1", "lang": "de"}, {"value": "ILCD format 1.1", "lang": "en"}], "type": "source data set", "refObjectId": "a97a0155-0234-4b87-b4ce-a45da52f2a40", "version": "01.00.000", "uri": "../sources/a97a0155-0234-4b87-b4ce-a45da52f2a40.xml"}, {"shortDescription": [{"value": "EPD-Datenformaterweiterungen v1.2", "lang": "de"}, {"value": "EPD Data Format Extensions v1.2", "lang": "en"}], "type": "source data set", "refObjectId": "a29449fd-aa2f-4de8-b5d7-4b06b43c6fde", "version": "00.01.000", "uri": "../sources/a29449fd-aa2f-4de8-b5d7-4b06b43c6fde.xml"}], "referenceToPersonOrEntityEnteringTheData": {"shortDescription": [{"value": "Sphera Solutions GmbH", "lang": "en"}], "type": "contact data set", "refObjectId": "d7fa0337-f279-430d-becf-7f3111a85010", "version": "24.01.000", "uri": "../contacts/d7fa0337-f279-430d-becf-7f3111a85010.xml"}}, "publicationAndOwnership": {"dataSetVersion": "20.24.070", "referenceToPrecedingDataSetVersion": [{"shortDescription": [{"value": "ETICS gluing and coating silicate dispersion plaster", "lang": "en"}], "type": "process data set", "refObjectId": "2d42602d-9913-43ed-8703-d953f7854bca", "uri": "https://www.oekobaudat.de/OEKOBAU.DAT/resource/processes/2d42602d-9913-43ed-8703-d953f7854bca?version=20.23.050"}], "referenceToRegistrationAuthority": {"shortDescription": [{"value": "Sphera Solutions GmbH", "lang": "en"}], "type": "contact data set", "refObjectId": "d7fa0337-f279-430d-becf-7f3111a85010", "version": "24.01.000", "uri": "../contacts/d7fa0337-f279-430d-becf-7f3111a85010.xml"}, "referenceToOwnershipOfDataSet": {"shortDescription": [{"value": "Sphera Solutions GmbH", "lang": "en"}], "type": "contact data set", "refObjectId": "d7fa0337-f279-430d-becf-7f3111a85010", "version": "24.01.000", "uri": "../contacts/d7fa0337-f279-430d-becf-7f3111a85010.xml"}, "copyright": true, "licenseType": "Free of charge for all users and uses", "accessRestrictions": [{"value": "The license conditions as stated on https://www.oekobaudat.de/apply.", "lang": "en"}, {"value": "Es gelten die Lizenzbedingungen wie sie auf https://www.oekobaudat.de/ genannt sind.", "lang": "de"}], "other": {"anies": [{"name": "referenceToPublisher", "value": {"shortDescription": [{"value": "BBSR", "lang": "en"}], "type": "contact data set", "refObjectId": "f11651e0-7877-11e3-981f-0800200c9a66", "version": "00.01.000", "uri": "../contacts/f11651e0-7877-11e3-981f-0800200c9a66.xml"}}]}}}, "exchanges": {"exchange": [{"dataSetInternalID": 100171, "referenceToFlowDataSet": {"shortDescription": [{"value": "ETICS gluing and coating silicate dispersion plaster", "lang": "en"}, {"value": "WDVS Verklebung und Beschichtung Silikat-Dispersionsputz", "lang": "de"}], "type": "flow data set", "refObjectId": "ea5f4834-53b5-4796-ada4-d24ed86316b3", "version": "24.01.000", "uri": "../flows/ea5f4834-53b5-4796-ada4-d24ed86316b3.xml"}, "meanAmount": 1.0, "referenceFlow": true, "resultingflowAmount": 1.0, "flowProperties": [{"name": [{"lang": "de", "value": "Masse"}, {"lang": "en", "value": "Mass"}], "uuid": "93a60a56-a3c8-11da-a746-0800200b9a66", "meanValue": 12.48}, {"name": [{"lang": "en", "value": "Area"}, {"lang": "de", "value": "Fläche"}], "uuid": "93a60a56-a3c8-19da-a746-0800200c9a66", "referenceFlowProperty": true, "meanValue": 1.0, "referenceUnit": "qm", "unitGroupUUID": "c20a03d7-bd90-4569-bc94-66cfd364dfc8"}], "materialProperties": [{"name": "grammage", "value": "12.48", "unit": "kg/m^2", "unitDescription": "kilograms per square meter"}], "typeOfFlow": "Product flow", "classification": {"classHierarchy": "Valuable substances / Systems / Assemblies / Building industry", "name": "GaBiCategories"}}, {"dataSetInternalID": 100172, "referenceToFlowDataSet": {"shortDescription": [{"value": "Use of renewable primary energy as energy carrier (PERE)", "lang": "en"}, {"value": "Erneuerbare Primärenergie als Energieträger (PERE)", "lang": "de"}], "type": "flow data set", "refObjectId": "20f32be5-0398-4288-9b6d-accddd195317", "version": "24.01.000", "uri": "../flows/20f32be5-0398-4288-9b6d-accddd195317.xml"}, "exchange direction": "INPUT", "other": {"anies": [{"value": "15.6864911580773", "module": "A1-A3"}, {"name": "referenceToUnitGroupDataSet", "value": {"shortDescription": [{"value": "MJ", "lang": "en"}], "type": "unit group data set", "refObjectId": "93a60a57-a3c8-11da-a746-0800200c9a66", "version": "03.00.000", "uri": "../unitgroups/93a60a57-a3c8-11da-a746-0800200c9a66.xml"}}, {"value": "0.0753777994346465", "module": "C2"}, {"value": "0", "module": "C3"}, {"value": "0.474231487391018", "module": "C4"}]}, "resolvedFlowVersion": "38.00.000", "flowProperties": [], "typeOfFlow": "Other flow", "classification": {"classHierarchy": "Quantities", "name": "GaBiCategories"}}, {"dataSetInternalID": 100173, "referenceToFlowDataSet": {"shortDescription": [{"value": "Use of renewable primary energy resources used as raw materials (PERM)", "lang": "en"}, {"value": "Erneuerbare Primärenergie zur stofflichen Nutzung (PERM)", "lang": "de"}], "type": "flow data set", "refObjectId": "fb3ec0de-548d-4508-aea5-00b73bf6f702", "version": "24.01.000", "uri": "../flows/fb3ec0de-548d-4508-aea5-00b73bf6f702.xml"}, "exchange direction": "INPUT", "other": {"anies": [{"value": "0", "module": "A1-A3"}, {"name": "referenceToUnitGroupDataSet", "value": {"shortDescription": [{"value": "MJ", "lang": "en"}], "type": "unit group data set", "refObjectId": "93a60a57-a3c8-11da-a746-0800200c9a66", "version": "03.00.000", "uri": "../unitgroups/93a60a57-a3c8-11da-a746-0800200c9a66.xml"}}, {"value": "0", "module": "C2"}, {"value": "0", "module": "C3"}, {"value": "0", "module": "C4"}]}, "resolvedFlowVersion": "38.00.000", "flowProperties": [], "typeOfFlow": "Other flow", "classification": {"classHierarchy": "Quantities", "name": "GaBiCategories"}}, {"dataSetInternalID": 100174, "referenceToFlowDataSet": {"shortDescription": [{"value": "Total use of renewable primary energy (PERT)", "lang": "en"}, {"value": "Total erneuerbare Primärenergie (PERT)", "lang": "de"}], "type": "flow data set", "refObjectId": "53f97275-fa8a-4cdd-9024-65936002acd0", "version": "24.01.000", "uri": "../flows/53f97275-fa8a-4cdd-9024-65936002acd0.xml"}, "exchange direction": "INPUT", "other": {"anies": [{"value": "15.6864911580773", "module": "A1-A3"}, {"name": "referenceToUnitGroupDataSet", "value": {"shortDescription": [{"value": "MJ", "lang": "en"}], "type": "unit group data set", "refObjectId": "93a60a57-a3c8-11da-a746-0800200c9a66", "version": "03.00.000", "uri": "../unitgroups/93a60a57-a3c8-11da-a746-0800200c9a66.xml"}}, {"value": "0.0753777994346465", "module": "C2"}, {"value": "0", "module": "C3"}, {"value": "0.474231487391018", "module": "C4"}]}, "resolvedFlowVersion": "38.00.000", "flowProperties": [], "typeOfFlow": "Other flow", "classification": {"classHierarchy": "Quantities / Environmental quantities / EPD EN 15804 / LCI indicators", "name": "GaBiCategories"}}, {"dataSetInternalID": 100175, "referenceToFlowDataSet": {"shortDescription": [{"value": "Use of non renewable primary energy as energy carrier (PENRE)", "lang": "en"}, {"value": "Nicht-erneuerbare Primärenergie als Energieträger (PENRE)", "lang": "de"}], "type": "flow data set", "refObjectId": "ac857178-2b45-46ec-892a-a9a4332f0372", "version": "24.01.000", "uri": "../flows/ac857178-2b45-46ec-892a-a9a4332f0372.xml"}, "exchange direction": "INPUT", "other": {"anies": [{"value": "62.1464951994127", "module": "A1-A3"}, {"name": "referenceToUnitGroupDataSet", "value": {"shortDescription": [{"value": "MJ", "lang": "en"}], "type": "unit group data set", "refObjectId": "93a60a57-a3c8-11da-a746-0800200c9a66", "version": "03.00.000", "uri": "../unitgroups/93a60a57-a3c8-11da-a746-0800200c9a66.xml"}}, {"value": "0.68111961642089", "module": "C2"}, {"value": "17.6", "module": "C3"}, {"value": "2.70829151446371", "module": "C4"}]}, "resolvedFlowVersion": "38.00.000", "flowProperties": [], "typeOfFlow": "Other flow", "classification": {"classHierarchy": "Quantities", "name": "GaBiCategories"}}, {"dataSetInternalID": 100176, "referenceToFlowDataSet": {"shortDescription": [{"value": "Use of non renewable primary energy resources used as raw materials (PENRM)", "lang": "en"}, {"value": "Nicht-erneuerbare Primärenergie zur stofflichen Nutzung (PENRM)", "lang": "de"}], "type": "flow data set", "refObjectId": "1421caa0-679d-4bf4-b282-0eb850ccae27", "version": "24.01.000", "uri": "../flows/1421caa0-679d-4bf4-b282-0eb850ccae27.xml"}, "exchange direction": "INPUT", "other": {"anies": [{"value": "16", "module": "A1-A3"}, {"name": "referenceToUnitGroupDataSet", "value": {"shortDescription": [{"value": "MJ", "lang": "en"}], "type": "unit group data set", "refObjectId": "93a60a57-a3c8-11da-a746-0800200c9a66", "version": "03.00.000", "uri": "../unitgroups/93a60a57-a3c8-11da-a746-0800200c9a66.xml"}}, {"value": "0", "module": "C2"}, {"value": "-16", "module": "C3"}, {"value": "0", "module": "C4"}]}, "resolvedFlowVersion": "38.00.000", "flowProperties": [], "typeOfFlow": "Other flow", "classification": {"classHierarchy": "Quantities", "name": "GaBiCategories"}}, {"dataSetInternalID": 100177, "referenceToFlowDataSet": {"shortDescription": [{"value": "Total use of non renewable primary energy resource (PENRT)", "lang": "en"}, {"value": "Total nicht-erneuerbare Primärenergie (PENRT)", "lang": "de"}], "type": "flow data set", "refObjectId": "06159210-646b-4c8d-8583-da9b3b95a6c1", "version": "24.01.000", "uri": "../flows/06159210-646b-4c8d-8583-da9b3b95a6c1.xml"}, "exchange direction": "INPUT", "other": {"anies": [{"value": "78.1464951994127", "module": "A1-A3"}, {"name": "referenceToUnitGroupDataSet", "value": {"shortDescription": [{"value": "MJ", "lang": "en"}], "type": "unit group data set", "refObjectId": "93a60a57-a3c8-11da-a746-0800200c9a66", "version": "03.00.000", "uri": "../unitgroups/93a60a57-a3c8-11da-a746-0800200c9a66.xml"}}, {"value": "0.68111961642089", "module": "C2"}, {"value": "1.6", "module": "C3"}, {"value": "2.70829151446371", "module": "C4"}]}, "resolvedFlowVersion": "38.00.000", "flowProperties": [], "typeOfFlow": "Other flow", "classification": {"classHierarchy": "Quantities / Environmental quantities / EPD EN 15804 / LCI indicators", "name": "GaBiCategories"}}, {"dataSetInternalID": 100178, "referenceToFlowDataSet": {"shortDescription": [{"value": "Use of secondary material (SM)", "lang": "en"}, {"value": "Einsatz von Sekundärstoffen (SM)", "lang": "de"}], "type": "flow data set", "refObjectId": "c6a1f35f-2d09-4f54-8dfb-97e502e1ce92", "version": "24.01.000", "uri": "../flows/c6a1f35f-2d09-4f54-8dfb-97e502e1ce92.xml"}, "exchange direction": "INPUT", "other": {"anies": [{"value": "0", "module": "A1-A3"}, {"name": "referenceToUnitGroupDataSet", "value": {"shortDescription": [{"value": "kg", "lang": "en"}], "type": "unit group data set", "refObjectId": "93a60a57-a4c8-11da-a746-0800200c9a66", "version": "03.00.000", "uri": "../unitgroups/93a60a57-a4c8-11da-a746-0800200c9a66.xml"}}, {"value": "0", "module": "C2"}, {"value": "0", "module": "C3"}, {"value": "0", "module": "C4"}]}, "resolvedFlowVersion": "38.00.000", "flowProperties": [], "typeOfFlow": "Other flow", "classification": {"classHierarchy": "Quantities / Environmental quantities / EPD EN 15804 / LCI indicators", "name": "GaBiCategories"}}, {"dataSetInternalID": 100179, "referenceToFlowDataSet": {"shortDescription": [{"value": "Use of renewable secondary fuels (SF)", "lang": "en"}, {"value": "Erneuerbare Sekundärbrennstoffe (SF)", "lang": "de"}], "type": "flow data set", "refObjectId": "64333088-a55f-4aa2-9a31-c10b07816787", "version": "24.01.000", "uri": "../flows/64333088-a55f-4aa2-9a31-c10b07816787.xml"}, "exchange direction": "INPUT", "other": {"anies": [{"value": "0", "module": "A1-A3"}, {"name": "referenceToUnitGroupDataSet", "value": {"shortDescription": [{"value": "MJ", "lang": "en"}], "type": "unit group data set", "refObjectId": "93a60a57-a3c8-11da-a746-0800200c9a66", "version": "03.00.000", "uri": "../unitgroups/93a60a57-a3c8-11da-a746-0800200c9a66.xml"}}, {"value": "0", "module": "C2"}, {"value": "0", "module": "C3"}, {"value": "0", "module": "C4"}]}, "resolvedFlowVersion": "38.00.000", "flowProperties": [], "typeOfFlow": "Other flow", "classification": {"classHierarchy": "Quantities / Environmental quantities / EPD EN 15804 / LCI indicators", "name": "GaBiCategories"}}, {"dataSetInternalID": 100180, "referenceToFlowDataSet": {"shortDescription": [{"value": "Use of non renewable secondary fuels (NRSF)", "lang": "en"}, {"value": "Nicht erneuerbare Sekundärbrennstoffe (NRSF)", "lang": "de"}], "type": "flow data set", "refObjectId": "89def144-d39a-4287-b86f-efde453ddcb2", "version": "24.01.000", "uri": "../flows/89def144-d39a-4287-b86f-efde453ddcb2.xml"}, "exchange direction": "INPUT", "other": {"anies": [{"value": "0", "module": "A1-A3"}, {"name": "referenceToUnitGroupDataSet", "value": {"shortDescription": [{"value": "MJ", "lang": "en"}], "type": "unit group data set", "refObjectId": "93a60a57-a3c8-11da-a746-0800200c9a66", "version": "03.00.000", "uri": "../unitgroups/93a60a57-a3c8-11da-a746-0800200c9a66.xml"}}, {"value": "0", "module": "C2"}, {"value": "0", "module": "C3"}, {"value": "0", "module": "C4"}]}, "resolvedFlowVersion": "38.00.000", "flowProperties": [], "typeOfFlow": "Other flow", "classification": {"classHierarchy": "Quantities / Environmental quantities / EPD EN 15804 / LCI indicators", "name": "GaBiCategories"}}, {"dataSetInternalID": 100181, "referenceToFlowDataSet": {"shortDescription": [{"value": "Net use of fresh water (FW)", "lang": "en"}, {"value": "Nettoeinsatz von Süßwasserressourcen (FW)", "lang": "de"}], "type": "flow data set", "refObjectId": "3cf952c8-f3a4-461d-8c96-96456ca62246", "version": "24.01.000", "uri": "../flows/3cf952c8-f3a4-461d-8c96-96456ca62246.xml"}, "exchange direction": "INPUT", "other": {"anies": [{"value": "0.035694101827105", "module": "A1-A3"}, {"name": "referenceToUnitGroupDataSet", "value": {"shortDescription": [{"value": "m3", "lang": "en"}], "type": "unit group data set", "refObjectId": "93a60a57-a3c8-12da-a746-0800200c9a66", "version": "03.00.000", "uri": "../unitgroups/93a60a57-a3c8-12da-a746-0800200c9a66.xml"}}, {"value": "7.0419149999008E-5", "module": "C2"}, {"value": "0", "module": "C3"}, {"value": "0.000716523670036463", "module": "C4"}]}, "resolvedFlowVersion": "38.00.000", "flowProperties": [], "typeOfFlow": "Other flow", "classification": {"classHierarchy": "Quantities / Environmental quantities / EPD EN 15804 / LCI indicators", "name": "GaBiCategories"}}, {"dataSetInternalID": 100182, "referenceToFlowDataSet": {"shortDescription": [{"value": "Hazardous waste disposed (HWD)", "lang": "en"}, {"value": "Gefährlicher Abfall zur Deponie (HWD)", "lang": "de"}], "type": "flow data set", "refObjectId": "430f9e0f-59b2-46a0-8e0d-55e0e84948fc", "version": "24.01.000", "uri": "../flows/430f9e0f-59b2-46a0-8e0d-55e0e84948fc.xml"}, "exchange direction": "OUTPUT", "other": {"anies": [{"value": "3.6823333402721E-8", "module": "A1-A3"}, {"name": "referenceToUnitGroupDataSet", "value": {"shortDescription": [{"value": "kg", "lang": "en"}], "type": "unit group data set", "refObjectId": "93a60a57-a4c8-11da-a746-0800200c9a66", "version": "03.00.000", "uri": "../unitgroups/93a60a57-a4c8-11da-a746-0800200c9a66.xml"}}, {"value": "3.3159697737572E-11", "module": "C2"}, {"value": "0", "module": "C3"}, {"value": "6.79676476518794E-10", "module": "C4"}]}, "resolvedFlowVersion": "38.00.000", "flowProperties": [], "typeOfFlow": "Other flow", "classification": {"classHierarchy": "Quantities / Environmental quantities / EPD EN 15804 / LCI indicators", "name": "GaBiCategories"}}, {"dataSetInternalID": 100183, "referenceToFlowDataSet": {"shortDescription": [{"value": "Non harzardous waste disposed (NHWD)", "lang": "en"}, {"value": "Entsorgter nicht gefährlicher Abfall (NHWD)", "lang": "de"}], "type": "flow data set", "refObjectId": "b29ef66b-e286-4afa-949f-62f1a7b4d7fa", "version": "24.01.000", "uri": "../flows/b29ef66b-e286-4afa-949f-62f1a7b4d7fa.xml"}, "exchange direction": "OUTPUT", "other": {"anies": [{"value": "1.67820464475141", "module": "A1-A3"}, {"name": "referenceToUnitGroupDataSet", "value": {"shortDescription": [{"value": "kg", "lang": "en"}], "type": "unit group data set", "refObjectId": "93a60a57-a4c8-11da-a746-0800200c9a66", "version": "03.00.000", "uri": "../unitgroups/93a60a57-a4c8-11da-a746-0800200c9a66.xml"}}, {"value": "0.000115161968266434", "module": "C2"}, {"value": "0", "module": "C3"}, {"value": "13.7367202533188", "module": "C4"}]}, "resolvedFlowVersion": "38.00.000", "flowProperties": [], "typeOfFlow": "Other flow", "classification": {"classHierarchy": "Quantities / Environmental quantities / EPD EN 15804 / LCI indicators", "name": "GaBiCategories"}}, {"dataSetInternalID": 100184, "referenceToFlowDataSet": {"shortDescription": [{"value": "Radioactive waste disposed (RWD)", "lang": "en"}, {"value": "Entsorgter radioaktiver Abfall (RWD)", "lang": "de"}], "type": "flow data set", "refObjectId": "3449546e-52ad-4b39-b809-9fb77cea8ff6", "version": "24.01.000", "uri": "../flows/3449546e-52ad-4b39-b809-9fb77cea8ff6.xml"}, "exchange direction": "OUTPUT", "other": {"anies": [{"value": "0.000969283420475354", "module": "A1-A3"}, {"name": "referenceToUnitGroupDataSet", "value": {"shortDescription": [{"value": "kg", "lang": "en"}], "type": "unit group data set", "refObjectId": "93a60a57-a4c8-11da-a746-0800200c9a66", "version": "03.00.000", "uri": "../unitgroups/93a60a57-a4c8-11da-a746-0800200c9a66.xml"}}, {"value": "1.08411647911948E-6", "module": "C2"}, {"value": "0", "module": "C3"}, {"value": "2.80195645724149E-5", "module": "C4"}]}, "resolvedFlowVersion": "38.00.000", "flowProperties": [], "typeOfFlow": "Other flow", "classification": {"classHierarchy": "Quantities / Environmental quantities / EPD EN 15804 / LCI indicators", "name": "GaBiCategories"}}, {"dataSetInternalID": 100185, "referenceToFlowDataSet": {"shortDescription": [{"value": "Components for re-use (CRU)", "lang": "en"}, {"value": "Komponenten für die Wiederverwendung (CRU)", "lang": "de"}], "type": "flow data set", "refObjectId": "a2b32f97-3fc7-4af2-b209-525bc6426f33", "version": "24.01.000", "uri": "../flows/a2b32f97-3fc7-4af2-b209-525bc6426f33.xml"}, "exchange direction": "OUTPUT", "other": {"anies": [{"value": "0", "module": "A1-A3"}, {"name": "referenceToUnitGroupDataSet", "value": {"shortDescription": [{"value": "kg", "lang": "en"}], "type": "unit group data set", "refObjectId": "93a60a57-a4c8-11da-a746-0800200c9a66", "version": "03.00.000", "uri": "../unitgroups/93a60a57-a4c8-11da-a746-0800200c9a66.xml"}}, {"value": "0", "module": "C2"}, {"value": "0", "module": "C3"}, {"value": "0", "module": "C4"}]}, "resolvedFlowVersion": "38.00.000", "flowProperties": [], "typeOfFlow": "Other flow", "classification": {"classHierarchy": "Quantities / Environmental quantities / EPD EN 15804 / LCI indicators", "name": "GaBiCategories"}}, {"dataSetInternalID": 100186, "referenceToFlowDataSet": {"shortDescription": [{"value": "Materials for recycling  (MFR)", "lang": "en"}, {"value": "Stoffe zum Recycling (MFR)", "lang": "de"}], "type": "flow data set", "refObjectId": "d7fe48a5-4103-49c8-9aae-b0b5dfdbd6ae", "version": "24.01.000", "uri": "../flows/d7fe48a5-4103-49c8-9aae-b0b5dfdbd6ae.xml"}, "exchange direction": "OUTPUT", "other": {"anies": [{"value": "0", "module": "A1-A3"}, {"name": "referenceToUnitGroupDataSet", "value": {"shortDescription": [{"value": "kg", "lang": "en"}], "type": "unit group data set", "refObjectId": "93a60a57-a4c8-11da-a746-0800200c9a66", "version": "03.00.000", "uri": "../unitgroups/93a60a57-a4c8-11da-a746-0800200c9a66.xml"}}, {"value": "0", "module": "C2"}, {"value": "0", "module": "C3"}, {"value": "0", "module": "C4"}]}, "resolvedFlowVersion": "38.00.000", "flowProperties": [], "typeOfFlow": "Other flow", "classification": {"classHierarchy": "Quantities / Environmental quantities / EPD EN 15804 / LCI indicators", "name": "GaBiCategories"}}, {"dataSetInternalID": 100187, "referenceToFlowDataSet": {"shortDescription": [{"value": "Materials for energy recovery (MER)", "lang": "en"}, {"value": "Stoffe für die Energierückgewinnung (MER)", "lang": "de"}], "type": "flow data set", "refObjectId": "59a9181c-3aaf-46ee-8b13-2b3723b6e447", "version": "24.01.000", "uri": "../flows/59a9181c-3aaf-46ee-8b13-2b3723b6e447.xml"}, "exchange direction": "OUTPUT", "other": {"anies": [{"value": "0", "module": "A1-A3"}, {"name": "referenceToUnitGroupDataSet", "value": {"shortDescription": [{"value": "kg", "lang": "en"}], "type": "unit group data set", "refObjectId": "93a60a57-a4c8-11da-a746-0800200c9a66", "version": "03.00.000", "uri": "../unitgroups/93a60a57-a4c8-11da-a746-0800200c9a66.xml"}}, {"value": "0", "module": "C2"}, {"value": "0", "module": "C3"}, {"value": "0", "module": "C4"}]}, "resolvedFlowVersion": "38.00.000", "flowProperties": [], "typeOfFlow": "Other flow", "classification": {"classHierarchy": "Quantities / Environmental quantities / EPD EN 15804 / LCI indicators", "name": "GaBiCategories"}}, {"dataSetInternalID": 100188, "referenceToFlowDataSet": {"shortDescription": [{"value": "Exported electrical energy (EEE)", "lang": "en"}, {"value": "Exportierte elektrische Energie (EEE)", "lang": "de"}], "type": "flow data set", "refObjectId": "4da0c987-2b76-40d6-9e9e-82a017aaaf29", "version": "24.01.000", "uri": "../flows/4da0c987-2b76-40d6-9e9e-82a017aaaf29.xml"}, "exchange direction": "OUTPUT", "other": {"anies": [{"value": "0", "module": "A1-A3"}, {"name": "referenceToUnitGroupDataSet", "value": {"shortDescription": [{"value": "MJ", "lang": "en"}], "type": "unit group data set", "refObjectId": "93a60a57-a3c8-11da-a746-0800200c9a66", "version": "03.00.000", "uri": "../unitgroups/93a60a57-a3c8-11da-a746-0800200c9a66.xml"}}, {"value": "0", "module": "C2"}, {"value": "0", "module": "C3"}, {"value": "0", "module": "C4"}]}, "resolvedFlowVersion": "38.00.000", "flowProperties": [], "typeOfFlow": "Other flow", "classification": {"classHierarchy": "Quantities / Environmental quantities / EPD EN 15804 / LCI indicators", "name": "GaBiCategories"}}, {"dataSetInternalID": 100189, "referenceToFlowDataSet": {"shortDescription": [{"value": "Exported thermal energy (EET)", "lang": "en"}, {"value": "Exportierte thermische Energie (EET)", "lang": "de"}], "type": "flow data set", "refObjectId": "98daf38a-7a79-46d3-9a37-2b7bd0955810", "version": "24.01.000", "uri": "../flows/98daf38a-7a79-46d3-9a37-2b7bd0955810.xml"}, "exchange direction": "OUTPUT", "other": {"anies": [{"value": "0", "module": "A1-A3"}, {"name": "referenceToUnitGroupDataSet", "value": {"shortDescription": [{"value": "MJ", "lang": "en"}], "type": "unit group data set", "refObjectId": "93a60a57-a3c8-11da-a746-0800200c9a66", "version": "03.00.000", "uri": "../unitgroups/93a60a57-a3c8-11da-a746-0800200c9a66.xml"}}, {"value": "0", "module": "C2"}, {"value": "0", "module": "C3"}, {"value": "0", "module": "C4"}]}, "resolvedFlowVersion": "38.00.000", "flowProperties": [], "typeOfFlow": "Other flow", "classification": {"classHierarchy": "Quantities / Environmental quantities / EPD EN 15804 / LCI indicators", "name": "GaBiCategories"}}]}, "LCIAResults": {"LCIAResult": [{"referenceToLCIAMethodDataSet": {"shortDescription": [{"value": "Climate change", "lang": "en"}, {"value": "Globales Erwärmungspotenzial - total (GWP-total)", "lang": "de"}], "type": "LCIA method data set", "refObjectId": "a7ea142a-9749-11ed-a8fc-0242ac120002", "version": "24.01.000", "uri": "../lciamethods/a7ea142a-9749-11ed-a8fc-0242ac120002.xml"}, "other": {"anies": [{"value": "5.74168897583028", "module": "A1-A3"}, {"value": "0.0531488928222515", "module": "C2"}, {"value": "0", "module": "C3"}, {"value": "0.207287547735772", "module": "C4"}, {"name": "referenceToUnitGroupDataSet", "value": {"shortDescription": [{"value": "kg CO2 eq.", "lang": "en"}], "type": "unit group data set", "refObjectId": "1ebf3012-d0db-4de2-aefd-ef30cedb0be1", "version": "25.00.000", "uri": "../unitgroups/1ebf3012-d0db-4de2-aefd-ef30cedb0be1.xml"}}]}}, {"referenceToLCIAMethodDataSet": {"shortDescription": [{"value": "Climate change-Fossil", "lang": "en"}, {"value": "Globales Erwärmungspotenzial - fossil (GWP-fossil)", "lang": "de"}], "type": "LCIA method data set", "refObjectId": "a7ea19c0-9749-11ed-a8fc-0242ac120002", "version": "24.01.000", "uri": "../lciamethods/a7ea19c0-9749-11ed-a8fc-0242ac120002.xml"}, "other": {"anies": [{"value": "5.80809886506469", "module": "A1-A3"}, {"value": "0.0518813192245589", "module": "C2"}, {"value": "0", "module": "C3"}, {"value": "0.205513274868015", "module": "C4"}, {"name": "referenceToUnitGroupDataSet", "value": {"shortDescription": [{"value": "kg CO2 eq.", "lang": "en"}], "type": "unit group data set", "refObjectId": "1ebf3012-d0db-4de2-aefd-ef30cedb0be1", "version": "25.00.000", "uri": "../unitgroups/1ebf3012-d0db-4de2-aefd-ef30cedb0be1.xml"}}]}}, {"referenceToLCIAMethodDataSet": {"shortDescription": [{"value": "Climate change-Biogenic", "lang": "en"}, {"value": "Globales Erwärmungspotenzial - biogen (GWP-biogenic)", "lang": "de"}], "type": "LCIA method data set", "refObjectId": "a7ea186c-9749-11ed-a8fc-0242ac120002", "version": "24.01.000", "uri": "../lciamethods/a7ea186c-9749-11ed-a8fc-0242ac120002.xml"}, "other": {"anies": [{"value": "-0.0757976845434151", "module": "A1-A3"}, {"value": "0.000269807069768947", "module": "C2"}, {"value": "0", "module": "C3"}, {"value": "0.000541608401747187", "module": "C4"}, {"name": "referenceToUnitGroupDataSet", "value": {"shortDescription": [{"value": "kg CO2 eq.", "lang": "en"}], "type": "unit group data set", "refObjectId": "1ebf3012-d0db-4de2-aefd-ef30cedb0be1", "version": "25.00.000", "uri": "../unitgroups/1ebf3012-d0db-4de2-aefd-ef30cedb0be1.xml"}}]}}, {"referenceToLCIAMethodDataSet": {"shortDescription": [{"value": "Climate change-Land use and land use change", "lang": "en"}, {"value": "Globales Erwärmungspotenzial - luluc (GWP-luluc)", "lang": "de"}], "type": "LCIA method data set", "refObjectId": "a7ea1ae2-9749-11ed-a8fc-0242ac120002", "version": "24.01.000", "uri": "../lciamethods/a7ea1ae2-9749-11ed-a8fc-0242ac120002.xml"}, "other": {"anies": [{"value": "0.00938779530900817", "module": "A1-A3"}, {"value": "0.00099776652792364", "module": "C2"}, {"value": "0", "module": "C3"}, {"value": "0.00123266446600972", "module": "C4"}, {"name": "referenceToUnitGroupDataSet", "value": {"shortDescription": [{"value": "kg CO2 eq.", "lang": "en"}], "type": "unit group data set", "refObjectId": "1ebf3012-d0db-4de2-aefd-ef30cedb0be1", "version": "25.00.000", "uri": "../unitgroups/1ebf3012-d0db-4de2-aefd-ef30cedb0be1.xml"}}]}}, {"referenceToLCIAMethodDataSet": {"shortDescription": [{"value": "Depletion potenzial of the stratospheric ozone layer (ODP)", "lang": "en"}, {"value": "Abbaupotenzial der stratosphärischen Ozonschicht (ODP)", "lang": "de"}], "type": "LCIA method data set", "refObjectId": "b5c629d6-def3-11e6-bf01-fe55135034f3", "version": "24.01.000", "uri": "../lciamethods/b5c629d6-def3-11e6-bf01-fe55135034f3.xml"}, "other": {"anies": [{"value": "2.56984200157504E-11", "module": "A1-A3"}, {"value": "1.63808165316175E-14", "module": "C2"}, {"value": "0", "module": "C3"}, {"value": "5.59944768000002E-13", "module": "C4"}, {"name": "referenceToUnitGroupDataSet", "value": {"shortDescription": [{"value": "kg CFC-11 eq.", "lang": "en"}], "type": "unit group data set", "refObjectId": "d9e957c9-7309-4474-bf3a-7777df6c4e5b", "version": "25.00.000", "uri": "../unitgroups/d9e957c9-7309-4474-bf3a-7777df6c4e5b.xml"}}]}}, {"referenceToLCIAMethodDataSet": {"shortDescription": [{"value": "Acidifcation potential, Accumulated Exceedance (AP)", "lang": "en"}, {"value": "Versauerungspotenzial, kumulierte Überschreitung (AP)", "lang": "de"}], "type": "LCIA method data set", "refObjectId": "b5c611c6-def3-11e6-bf01-fe55135034f3", "version": "24.01.000", "uri": "../lciamethods/b5c611c6-def3-11e6-bf01-fe55135034f3.xml"}, "other": {"anies": [{"value": "0.0140107252739293", "module": "A1-A3"}, {"value": "6.84798719820278E-5", "module": "C2"}, {"value": "0", "module": "C3"}, {"value": "0.00145863281871732", "module": "C4"}, {"name": "referenceToUnitGroupDataSet", "value": {"shortDescription": [{"value": "Mole of H+ eq.", "lang": "en"}], "type": "unit group data set", "refObjectId": "42e089ac-92bf-4bf2-8ca1-5fc40d18f2ed", "version": "00.01.000", "uri": "../unitgroups/42e089ac-92bf-4bf2-8ca1-5fc40d18f2ed.xml"}}]}}, {"referenceToLCIAMethodDataSet": {"shortDescription": [{"value": "Eutrophication, freshwater", "lang": "en"}, {"value": "Eutrophierungspotenzial - Süßwasser (EP-freshwater)", "lang": "de"}], "type": "LCIA method data set", "refObjectId": "b53ec18f-7377-4ad3-86eb-cc3f4f276b2b", "version": "24.01.000", "uri": "../lciamethods/b53ec18f-7377-4ad3-86eb-cc3f4f276b2b.xml"}, "other": {"anies": [{"value": "1.78784989572975E-5", "module": "A1-A3"}, {"value": "1.41262381542658E-7", "module": "C2"}, {"value": "0", "module": "C3"}, {"value": "4.6817638408653E-7", "module": "C4"}, {"name": "referenceToUnitGroupDataSet", "value": {"shortDescription": [{"value": "kg P eq.", "lang": "en"}], "type": "unit group data set", "refObjectId": "0429039d-a61d-4590-ba67-aa4a20a810a1", "version": "25.00.000", "uri": "../unitgroups/0429039d-a61d-4590-ba67-aa4a20a810a1.xml"}}]}}, {"referenceToLCIAMethodDataSet": {"shortDescription": [{"value": "Eutrophication marine", "lang": "en"}, {"value": "Eutrophierungspotenzial - Salzwasser (EP-marine)", "lang": "de"}], "type": "LCIA method data set", "refObjectId": "b5c619fa-def3-11e6-bf01-fe55135034f3", "version": "24.01.000", "uri": "../lciamethods/b5c619fa-def3-11e6-bf01-fe55135034f3.xml"}, "other": {"anies": [{"value": "0.00426845736180918", "module": "A1-A3"}, {"value": "2.42620685024806E-5", "module": "C2"}, {"value": "0", "module": "C3"}, {"value": "0.000375523434726528", "module": "C4"}, {"name": "referenceToUnitGroupDataSet", "value": {"shortDescription": [{"value": "kg N eq.", "lang": "en"}], "type": "unit group data set", "refObjectId": "d05bb823-ecdf-4686-8c40-bf1d9257859f", "version": "00.00.003", "uri": "../unitgroups/d05bb823-ecdf-4686-8c40-bf1d9257859f.xml"}}]}}, {"referenceToLCIAMethodDataSet": {"shortDescription": [{"value": "Eutrophication, terrestrial", "lang": "en"}, {"value": "Eutrophierungspotenzial - Land (EP-terrestrial)", "lang": "de"}], "type": "LCIA method data set", "refObjectId": "b5c614d2-def3-11e6-bf01-fe55135034f3", "version": "24.01.000", "uri": "../lciamethods/b5c614d2-def3-11e6-bf01-fe55135034f3.xml"}, "other": {"anies": [{"value": "0.0475209694951833", "module": "A1-A3"}, {"value": "0.000294794618910342", "module": "C2"}, {"value": "0", "module": "C3"}, {"value": "0.00413510734070132", "module": "C4"}, {"name": "referenceToUnitGroupDataSet", "value": {"shortDescription": [{"value": "Mole of N eq.", "lang": "en"}], "type": "unit group data set", "refObjectId": "71b4d617-0ec9-4d3f-b65e-e438940c2401", "version": "00.00.003", "uri": "../unitgroups/71b4d617-0ec9-4d3f-b65e-e438940c2401.xml"}}]}}, {"referenceToLCIAMethodDataSet": {"shortDescription": [{"value": "Photochemical Ozone Creation Potential  (POCP)", "lang": "en"}, {"value": "Bildungspotenzial für troposphärisches Ozon (POCP)", "lang": "de"}], "type": "LCIA method data set", "refObjectId": "b5c610fe-def3-11e6-bf01-fe55135034f3", "version": "24.01.000", "uri": "../lciamethods/b5c610fe-def3-11e6-bf01-fe55135034f3.xml"}, "other": {"anies": [{"value": "0.0165191267254228", "module": "A1-A3"}, {"value": "6.64821991643519E-5", "module": "C2"}, {"value": "0", "module": "C3"}, {"value": "0.00114912532040415", "module": "C4"}, {"name": "referenceToUnitGroupDataSet", "value": {"shortDescription": [{"value": "kg NMVOC eq.", "lang": "en"}], "type": "unit group data set", "refObjectId": "d27c25f8-fbc1-44c6-b47b-4adbae4199c6", "version": "00.00.003", "uri": "../unitgroups/d27c25f8-fbc1-44c6-b47b-4adbae4199c6.xml"}}]}}, {"referenceToLCIAMethodDataSet": {"shortDescription": [{"value": "Resource use, minerals and metals", "lang": "en"}, {"value": "Potenzial für die Verknappung abiotischer Ressourcen  nicht fossile Ressourcen (ADPE)", "lang": "de"}], "type": "LCIA method data set", "refObjectId": "b2ad6494-c78d-11e6-9d9d-cec0c932ce01", "version": "24.01.000", "uri": "../lciamethods/b2ad6494-c78d-11e6-9d9d-cec0c932ce01.xml"}, "other": {"anies": [{"value": "1.57121800491952E-5", "module": "A1-A3"}, {"value": "8.80305384354948E-9", "module": "C2"}, {"value": "0", "module": "C3"}, {"value": "1.31333470574184E-8", "module": "C4"}, {"name": "referenceToUnitGroupDataSet", "value": {"shortDescription": [{"value": "kg Sb eq.", "lang": "en"}], "type": "unit group data set", "refObjectId": "54ccd2d9-a32a-4fc2-923d-f2c8c93e89d4", "version": "25.00.000", "uri": "../unitgroups/54ccd2d9-a32a-4fc2-923d-f2c8c93e89d4.xml"}}]}}, {"referenceToLCIAMethodDataSet": {"shortDescription": [{"value": "Resource use, fossils", "lang": "en"}, {"value": "Potenzial für die Verknappung abiotischer Ressourcen  fossile Brennstoffe (ADPF)", "lang": "de"}], "type": "LCIA method data set", "refObjectId": "b2ad6110-c78d-11e6-9d9d-cec0c932ce01", "version": "24.01.000", "uri": "../lciamethods/b2ad6110-c78d-11e6-9d9d-cec0c932ce01.xml"}, "other": {"anies": [{"value": "79.7457341112925", "module": "A1-A3"}, {"value": "0.68110788372197", "module": "C2"}, {"value": "0", "module": "C3"}, {"value": "2.70825759689803", "module": "C4"}, {"name": "referenceToUnitGroupDataSet", "value": {"shortDescription": [{"value": "MJ", "lang": "en"}], "type": "unit group data set", "refObjectId": "93a60a57-a3c8-11da-a746-0800200c9a66", "version": "02.00.000", "uri": "../unitgroups/93a60a57-a3c8-11da-a746-0800200c9a66.xml"}}]}}, {"referenceToLCIAMethodDataSet": {"shortDescription": [{"value": "Water use", "lang": "en"}, {"value": "Wasser-Entzugspotenzial (Benutzer) (WDP)", "lang": "de"}], "type": "LCIA method data set", "refObjectId": "b2ad66ce-c78d-11e6-9d9d-cec0c932ce01", "version": "24.01.000", "uri": "../lciamethods/b2ad66ce-c78d-11e6-9d9d-cec0c932ce01.xml"}, "other": {"anies": [{"value": "0.954707449909742", "module": "A1-A3"}, {"value": "0.000371805887092485", "module": "C2"}, {"value": "0", "module": "C3"}, {"value": "0.0234461105832539", "module": "C4"}, {"name": "referenceToUnitGroupDataSet", "value": {"shortDescription": [{"value": "m³ world equiv.", "lang": "en"}], "type": "unit group data set", "refObjectId": "6ae2df01-888e-46c8-b17d-49fa3869b476", "version": "00.00.003", "uri": "../unitgroups/6ae2df01-888e-46c8-b17d-49fa3869b476.xml"}}]}}]}, "otherAttributes": {"{http://www.indata.network/EPD/2019}epd-version": "1.2"}, "version": "1.1", "locations": "../ILCDLocations.xml"}