{"processInformation": {"dataSetInformation": {"UUID": "bcf5c14e-f6c1-4a53-bfd0-32dd6b493028", "name": {"baseName": [{"value": "Baufritz GaBi HOIZ Hobelspandämmung NA", "lang": "de"}, {"value": "Baufritz GaBi HOIZ wood chip insulation - reissue", "lang": "en"}], "functionalUnitFlowProperties": [{"value": "70 kg/m³", "lang": "de"}]}, "synonyms": [{"value": "Holzspandämmung, Holzdämmung, Holzfaserdämmung", "lang": "de"}, {"value": "Wood chip insulation, wood insulation, wood fibre insulation", "lang": "en"}], "classificationInformation": {"classification": [{"class": [{"value": "Dämmstoffe", "level": 0, "classId": "2"}, {"value": "Holzfasern", "level": 1, "classId": "2.10"}, {"value": "Holzfasern und Holzspäne, lose", "level": 2, "classId": "2.10.02"}], "name": "OEKOBAU.DAT"}]}, "generalComment": [{"value": "Die gegenständliche EPD bezieht sich auf das Produkt HOIZ - Hobelspandämmung, hergestellt in dem Werk in 87746 Erkheim, Deutschland.\r\nDie HOIZ - Hobelspandämmung wird als Wärme- und Schalldämmstoff für Dächer, Decken und Wände als nicht belastbare Hohlraumdämmung im Holzbau eingesetzt. Generell können jedoch alle Hohlräume von Bauteilen (auch Stahlkonstruktionen) damit gedämmt bzw. akustisch gedämmt werden.\r\nDer Dämmstoff wird jedoch nur werksintern in Fertigteile verbaut und nicht als „reiner“ Dämmstoff separat ausgeliefert.", "lang": "de"}, {"value": "This EPD refers to the product HOIZ - wood shaving insulation, manufactured at the factory in 87746 Erkheim, Germany. \nHOIZ - wood shaving insulation is used as thermal and sound insulation for roofs, ceilings and walls as non-load-bearing cavity insulation in timber construction. In general all cavities in building components (including steel structures) could be insulated or acoustically insulated with it. \nHowever, the insulation material is only installed in prefabricated parts in-house and is not delivered separately as a ‘pure’ insulation material.", "lang": "en"}], "other": {"anies": [{"margins": 0.0, "description": [{"value": "keine", "lang": "de"}, {"value": "none", "lang": "en"}]}, {"scenario": [{"description": [{"value": "Thermische Verwertung", "lang": "de"}], "name": "Thermische Verwertung", "default": true}]}, "<ns11:modules xmlns:ns11=\"http://openlca.org/epd_ilcd\" xmlns=\"http://lca.jrc.it/ILCD/Process\" xmlns:c=\"http://lca.jrc.it/ILCD/Contact\" xmlns:common=\"http://lca.jrc.it/ILCD/Common\" xmlns:epd=\"http://www.iai.kit.edu/EPD/2013\" xmlns:epd2=\"http://www.indata.network/EPD/2019\" xmlns:f=\"http://lca.jrc.it/ILCD/Flow\" xmlns:fp=\"http://lca.jrc.it/ILCD/FlowProperty\" xmlns:m=\"http://lca.jrc.it/ILCD/LCIAMethod\" xmlns:ns9=\"http://www.okworx.com/ILCD/Extensions/2018/Profile\" xmlns:s=\"http://lca.jrc.it/ILCD/Source\" xmlns:u=\"http://lca.jrc.it/ILCD/UnitGroup\" name=\"A1\"/>", "<ns11:modules xmlns:ns11=\"http://openlca.org/epd_ilcd\" xmlns=\"http://lca.jrc.it/ILCD/Process\" xmlns:c=\"http://lca.jrc.it/ILCD/Contact\" xmlns:common=\"http://lca.jrc.it/ILCD/Common\" xmlns:epd=\"http://www.iai.kit.edu/EPD/2013\" xmlns:epd2=\"http://www.indata.network/EPD/2019\" xmlns:f=\"http://lca.jrc.it/ILCD/Flow\" xmlns:fp=\"http://lca.jrc.it/ILCD/FlowProperty\" xmlns:m=\"http://lca.jrc.it/ILCD/LCIAMethod\" xmlns:ns9=\"http://www.okworx.com/ILCD/Extensions/2018/Profile\" xmlns:s=\"http://lca.jrc.it/ILCD/Source\" xmlns:u=\"http://lca.jrc.it/ILCD/UnitGroup\" name=\"A1-A3\"/>", "<ns11:modules xmlns:ns11=\"http://openlca.org/epd_ilcd\" xmlns=\"http://lca.jrc.it/ILCD/Process\" xmlns:c=\"http://lca.jrc.it/ILCD/Contact\" xmlns:common=\"http://lca.jrc.it/ILCD/Common\" xmlns:epd=\"http://www.iai.kit.edu/EPD/2013\" xmlns:epd2=\"http://www.indata.network/EPD/2019\" xmlns:f=\"http://lca.jrc.it/ILCD/Flow\" xmlns:fp=\"http://lca.jrc.it/ILCD/FlowProperty\" xmlns:m=\"http://lca.jrc.it/ILCD/LCIAMethod\" xmlns:ns9=\"http://www.okworx.com/ILCD/Extensions/2018/Profile\" xmlns:s=\"http://lca.jrc.it/ILCD/Source\" xmlns:u=\"http://lca.jrc.it/ILCD/UnitGroup\" name=\"A2\"/>", "<ns11:modules xmlns:ns11=\"http://openlca.org/epd_ilcd\" xmlns=\"http://lca.jrc.it/ILCD/Process\" xmlns:c=\"http://lca.jrc.it/ILCD/Contact\" xmlns:common=\"http://lca.jrc.it/ILCD/Common\" xmlns:epd=\"http://www.iai.kit.edu/EPD/2013\" xmlns:epd2=\"http://www.indata.network/EPD/2019\" xmlns:f=\"http://lca.jrc.it/ILCD/Flow\" xmlns:fp=\"http://lca.jrc.it/ILCD/FlowProperty\" xmlns:m=\"http://lca.jrc.it/ILCD/LCIAMethod\" xmlns:ns9=\"http://www.okworx.com/ILCD/Extensions/2018/Profile\" xmlns:s=\"http://lca.jrc.it/ILCD/Source\" xmlns:u=\"http://lca.jrc.it/ILCD/UnitGroup\" name=\"A3\"/>", "<ns11:modules xmlns:ns11=\"http://openlca.org/epd_ilcd\" xmlns=\"http://lca.jrc.it/ILCD/Process\" xmlns:c=\"http://lca.jrc.it/ILCD/Contact\" xmlns:common=\"http://lca.jrc.it/ILCD/Common\" xmlns:epd=\"http://www.iai.kit.edu/EPD/2013\" xmlns:epd2=\"http://www.indata.network/EPD/2019\" xmlns:f=\"http://lca.jrc.it/ILCD/Flow\" xmlns:fp=\"http://lca.jrc.it/ILCD/FlowProperty\" xmlns:m=\"http://lca.jrc.it/ILCD/LCIAMethod\" xmlns:ns9=\"http://www.okworx.com/ILCD/Extensions/2018/Profile\" xmlns:s=\"http://lca.jrc.it/ILCD/Source\" xmlns:u=\"http://lca.jrc.it/ILCD/UnitGroup\" name=\"A4\"/>", "<ns11:modules xmlns:ns11=\"http://openlca.org/epd_ilcd\" xmlns=\"http://lca.jrc.it/ILCD/Process\" xmlns:c=\"http://lca.jrc.it/ILCD/Contact\" xmlns:common=\"http://lca.jrc.it/ILCD/Common\" xmlns:epd=\"http://www.iai.kit.edu/EPD/2013\" xmlns:epd2=\"http://www.indata.network/EPD/2019\" xmlns:f=\"http://lca.jrc.it/ILCD/Flow\" xmlns:fp=\"http://lca.jrc.it/ILCD/FlowProperty\" xmlns:m=\"http://lca.jrc.it/ILCD/LCIAMethod\" xmlns:ns9=\"http://www.okworx.com/ILCD/Extensions/2018/Profile\" xmlns:s=\"http://lca.jrc.it/ILCD/Source\" xmlns:u=\"http://lca.jrc.it/ILCD/UnitGroup\" name=\"A5\"/>", "<ns11:modules xmlns:ns11=\"http://openlca.org/epd_ilcd\" xmlns=\"http://lca.jrc.it/ILCD/Process\" xmlns:c=\"http://lca.jrc.it/ILCD/Contact\" xmlns:common=\"http://lca.jrc.it/ILCD/Common\" xmlns:epd=\"http://www.iai.kit.edu/EPD/2013\" xmlns:epd2=\"http://www.indata.network/EPD/2019\" xmlns:f=\"http://lca.jrc.it/ILCD/Flow\" xmlns:fp=\"http://lca.jrc.it/ILCD/FlowProperty\" xmlns:m=\"http://lca.jrc.it/ILCD/LCIAMethod\" xmlns:ns9=\"http://www.okworx.com/ILCD/Extensions/2018/Profile\" xmlns:s=\"http://lca.jrc.it/ILCD/Source\" xmlns:u=\"http://lca.jrc.it/ILCD/UnitGroup\" name=\"B1\"/>", "<ns11:modules xmlns:ns11=\"http://openlca.org/epd_ilcd\" xmlns=\"http://lca.jrc.it/ILCD/Process\" xmlns:c=\"http://lca.jrc.it/ILCD/Contact\" xmlns:common=\"http://lca.jrc.it/ILCD/Common\" xmlns:epd=\"http://www.iai.kit.edu/EPD/2013\" xmlns:epd2=\"http://www.indata.network/EPD/2019\" xmlns:f=\"http://lca.jrc.it/ILCD/Flow\" xmlns:fp=\"http://lca.jrc.it/ILCD/FlowProperty\" xmlns:m=\"http://lca.jrc.it/ILCD/LCIAMethod\" xmlns:ns9=\"http://www.okworx.com/ILCD/Extensions/2018/Profile\" xmlns:s=\"http://lca.jrc.it/ILCD/Source\" xmlns:u=\"http://lca.jrc.it/ILCD/UnitGroup\" name=\"B2\"/>", "<ns11:modules xmlns:ns11=\"http://openlca.org/epd_ilcd\" xmlns=\"http://lca.jrc.it/ILCD/Process\" xmlns:c=\"http://lca.jrc.it/ILCD/Contact\" xmlns:common=\"http://lca.jrc.it/ILCD/Common\" xmlns:epd=\"http://www.iai.kit.edu/EPD/2013\" xmlns:epd2=\"http://www.indata.network/EPD/2019\" xmlns:f=\"http://lca.jrc.it/ILCD/Flow\" xmlns:fp=\"http://lca.jrc.it/ILCD/FlowProperty\" xmlns:m=\"http://lca.jrc.it/ILCD/LCIAMethod\" xmlns:ns9=\"http://www.okworx.com/ILCD/Extensions/2018/Profile\" xmlns:s=\"http://lca.jrc.it/ILCD/Source\" xmlns:u=\"http://lca.jrc.it/ILCD/UnitGroup\" name=\"B3\"/>", "<ns11:modules xmlns:ns11=\"http://openlca.org/epd_ilcd\" xmlns=\"http://lca.jrc.it/ILCD/Process\" xmlns:c=\"http://lca.jrc.it/ILCD/Contact\" xmlns:common=\"http://lca.jrc.it/ILCD/Common\" xmlns:epd=\"http://www.iai.kit.edu/EPD/2013\" xmlns:epd2=\"http://www.indata.network/EPD/2019\" xmlns:f=\"http://lca.jrc.it/ILCD/Flow\" xmlns:fp=\"http://lca.jrc.it/ILCD/FlowProperty\" xmlns:m=\"http://lca.jrc.it/ILCD/LCIAMethod\" xmlns:ns9=\"http://www.okworx.com/ILCD/Extensions/2018/Profile\" xmlns:s=\"http://lca.jrc.it/ILCD/Source\" xmlns:u=\"http://lca.jrc.it/ILCD/UnitGroup\" name=\"B4\"/>", "<ns11:modules xmlns:ns11=\"http://openlca.org/epd_ilcd\" xmlns=\"http://lca.jrc.it/ILCD/Process\" xmlns:c=\"http://lca.jrc.it/ILCD/Contact\" xmlns:common=\"http://lca.jrc.it/ILCD/Common\" xmlns:epd=\"http://www.iai.kit.edu/EPD/2013\" xmlns:epd2=\"http://www.indata.network/EPD/2019\" xmlns:f=\"http://lca.jrc.it/ILCD/Flow\" xmlns:fp=\"http://lca.jrc.it/ILCD/FlowProperty\" xmlns:m=\"http://lca.jrc.it/ILCD/LCIAMethod\" xmlns:ns9=\"http://www.okworx.com/ILCD/Extensions/2018/Profile\" xmlns:s=\"http://lca.jrc.it/ILCD/Source\" xmlns:u=\"http://lca.jrc.it/ILCD/UnitGroup\" name=\"B4\" scenario=\"Thermische Verwertung\"/>", "<ns11:modules xmlns:ns11=\"http://openlca.org/epd_ilcd\" xmlns=\"http://lca.jrc.it/ILCD/Process\" xmlns:c=\"http://lca.jrc.it/ILCD/Contact\" xmlns:common=\"http://lca.jrc.it/ILCD/Common\" xmlns:epd=\"http://www.iai.kit.edu/EPD/2013\" xmlns:epd2=\"http://www.indata.network/EPD/2019\" xmlns:f=\"http://lca.jrc.it/ILCD/Flow\" xmlns:fp=\"http://lca.jrc.it/ILCD/FlowProperty\" xmlns:m=\"http://lca.jrc.it/ILCD/LCIAMethod\" xmlns:ns9=\"http://www.okworx.com/ILCD/Extensions/2018/Profile\" xmlns:s=\"http://lca.jrc.it/ILCD/Source\" xmlns:u=\"http://lca.jrc.it/ILCD/UnitGroup\" name=\"B5\"/>", "<ns11:modules xmlns:ns11=\"http://openlca.org/epd_ilcd\" xmlns=\"http://lca.jrc.it/ILCD/Process\" xmlns:c=\"http://lca.jrc.it/ILCD/Contact\" xmlns:common=\"http://lca.jrc.it/ILCD/Common\" xmlns:epd=\"http://www.iai.kit.edu/EPD/2013\" xmlns:epd2=\"http://www.indata.network/EPD/2019\" xmlns:f=\"http://lca.jrc.it/ILCD/Flow\" xmlns:fp=\"http://lca.jrc.it/ILCD/FlowProperty\" xmlns:m=\"http://lca.jrc.it/ILCD/LCIAMethod\" xmlns:ns9=\"http://www.okworx.com/ILCD/Extensions/2018/Profile\" xmlns:s=\"http://lca.jrc.it/ILCD/Source\" xmlns:u=\"http://lca.jrc.it/ILCD/UnitGroup\" name=\"B6\"/>", "<ns11:modules xmlns:ns11=\"http://openlca.org/epd_ilcd\" xmlns=\"http://lca.jrc.it/ILCD/Process\" xmlns:c=\"http://lca.jrc.it/ILCD/Contact\" xmlns:common=\"http://lca.jrc.it/ILCD/Common\" xmlns:epd=\"http://www.iai.kit.edu/EPD/2013\" xmlns:epd2=\"http://www.indata.network/EPD/2019\" xmlns:f=\"http://lca.jrc.it/ILCD/Flow\" xmlns:fp=\"http://lca.jrc.it/ILCD/FlowProperty\" xmlns:m=\"http://lca.jrc.it/ILCD/LCIAMethod\" xmlns:ns9=\"http://www.okworx.com/ILCD/Extensions/2018/Profile\" xmlns:s=\"http://lca.jrc.it/ILCD/Source\" xmlns:u=\"http://lca.jrc.it/ILCD/UnitGroup\" name=\"B7\"/>", "<ns11:modules xmlns:ns11=\"http://openlca.org/epd_ilcd\" xmlns=\"http://lca.jrc.it/ILCD/Process\" xmlns:c=\"http://lca.jrc.it/ILCD/Contact\" xmlns:common=\"http://lca.jrc.it/ILCD/Common\" xmlns:epd=\"http://www.iai.kit.edu/EPD/2013\" xmlns:epd2=\"http://www.indata.network/EPD/2019\" xmlns:f=\"http://lca.jrc.it/ILCD/Flow\" xmlns:fp=\"http://lca.jrc.it/ILCD/FlowProperty\" xmlns:m=\"http://lca.jrc.it/ILCD/LCIAMethod\" xmlns:ns9=\"http://www.okworx.com/ILCD/Extensions/2018/Profile\" xmlns:s=\"http://lca.jrc.it/ILCD/Source\" xmlns:u=\"http://lca.jrc.it/ILCD/UnitGroup\" name=\"C1\" scenario=\"0\"/>", "<ns11:modules xmlns:ns11=\"http://openlca.org/epd_ilcd\" xmlns=\"http://lca.jrc.it/ILCD/Process\" xmlns:c=\"http://lca.jrc.it/ILCD/Contact\" xmlns:common=\"http://lca.jrc.it/ILCD/Common\" xmlns:epd=\"http://www.iai.kit.edu/EPD/2013\" xmlns:epd2=\"http://www.indata.network/EPD/2019\" xmlns:f=\"http://lca.jrc.it/ILCD/Flow\" xmlns:fp=\"http://lca.jrc.it/ILCD/FlowProperty\" xmlns:m=\"http://lca.jrc.it/ILCD/LCIAMethod\" xmlns:ns9=\"http://www.okworx.com/ILCD/Extensions/2018/Profile\" xmlns:s=\"http://lca.jrc.it/ILCD/Source\" xmlns:u=\"http://lca.jrc.it/ILCD/UnitGroup\" name=\"C1\" scenario=\"Thermische Verwertung\"/>", "<ns11:modules xmlns:ns11=\"http://openlca.org/epd_ilcd\" xmlns=\"http://lca.jrc.it/ILCD/Process\" xmlns:c=\"http://lca.jrc.it/ILCD/Contact\" xmlns:common=\"http://lca.jrc.it/ILCD/Common\" xmlns:epd=\"http://www.iai.kit.edu/EPD/2013\" xmlns:epd2=\"http://www.indata.network/EPD/2019\" xmlns:f=\"http://lca.jrc.it/ILCD/Flow\" xmlns:fp=\"http://lca.jrc.it/ILCD/FlowProperty\" xmlns:m=\"http://lca.jrc.it/ILCD/LCIAMethod\" xmlns:ns9=\"http://www.okworx.com/ILCD/Extensions/2018/Profile\" xmlns:s=\"http://lca.jrc.it/ILCD/Source\" xmlns:u=\"http://lca.jrc.it/ILCD/UnitGroup\" name=\"C2\" scenario=\"0\"/>", "<ns11:modules xmlns:ns11=\"http://openlca.org/epd_ilcd\" xmlns=\"http://lca.jrc.it/ILCD/Process\" xmlns:c=\"http://lca.jrc.it/ILCD/Contact\" xmlns:common=\"http://lca.jrc.it/ILCD/Common\" xmlns:epd=\"http://www.iai.kit.edu/EPD/2013\" xmlns:epd2=\"http://www.indata.network/EPD/2019\" xmlns:f=\"http://lca.jrc.it/ILCD/Flow\" xmlns:fp=\"http://lca.jrc.it/ILCD/FlowProperty\" xmlns:m=\"http://lca.jrc.it/ILCD/LCIAMethod\" xmlns:ns9=\"http://www.okworx.com/ILCD/Extensions/2018/Profile\" xmlns:s=\"http://lca.jrc.it/ILCD/Source\" xmlns:u=\"http://lca.jrc.it/ILCD/UnitGroup\" name=\"C2\" scenario=\"Thermische Verwertung\"/>", "<ns11:modules xmlns:ns11=\"http://openlca.org/epd_ilcd\" xmlns=\"http://lca.jrc.it/ILCD/Process\" xmlns:c=\"http://lca.jrc.it/ILCD/Contact\" xmlns:common=\"http://lca.jrc.it/ILCD/Common\" xmlns:epd=\"http://www.iai.kit.edu/EPD/2013\" xmlns:epd2=\"http://www.indata.network/EPD/2019\" xmlns:f=\"http://lca.jrc.it/ILCD/Flow\" xmlns:fp=\"http://lca.jrc.it/ILCD/FlowProperty\" xmlns:m=\"http://lca.jrc.it/ILCD/LCIAMethod\" xmlns:ns9=\"http://www.okworx.com/ILCD/Extensions/2018/Profile\" xmlns:s=\"http://lca.jrc.it/ILCD/Source\" xmlns:u=\"http://lca.jrc.it/ILCD/UnitGroup\" name=\"C3\" scenario=\"0\"/>", "<ns11:modules xmlns:ns11=\"http://openlca.org/epd_ilcd\" xmlns=\"http://lca.jrc.it/ILCD/Process\" xmlns:c=\"http://lca.jrc.it/ILCD/Contact\" xmlns:common=\"http://lca.jrc.it/ILCD/Common\" xmlns:epd=\"http://www.iai.kit.edu/EPD/2013\" xmlns:epd2=\"http://www.indata.network/EPD/2019\" xmlns:f=\"http://lca.jrc.it/ILCD/Flow\" xmlns:fp=\"http://lca.jrc.it/ILCD/FlowProperty\" xmlns:m=\"http://lca.jrc.it/ILCD/LCIAMethod\" xmlns:ns9=\"http://www.okworx.com/ILCD/Extensions/2018/Profile\" xmlns:s=\"http://lca.jrc.it/ILCD/Source\" xmlns:u=\"http://lca.jrc.it/ILCD/UnitGroup\" name=\"C3\" scenario=\"Thermische Verwertung\"/>", "<ns11:modules xmlns:ns11=\"http://openlca.org/epd_ilcd\" xmlns=\"http://lca.jrc.it/ILCD/Process\" xmlns:c=\"http://lca.jrc.it/ILCD/Contact\" xmlns:common=\"http://lca.jrc.it/ILCD/Common\" xmlns:epd=\"http://www.iai.kit.edu/EPD/2013\" xmlns:epd2=\"http://www.indata.network/EPD/2019\" xmlns:f=\"http://lca.jrc.it/ILCD/Flow\" xmlns:fp=\"http://lca.jrc.it/ILCD/FlowProperty\" xmlns:m=\"http://lca.jrc.it/ILCD/LCIAMethod\" xmlns:ns9=\"http://www.okworx.com/ILCD/Extensions/2018/Profile\" xmlns:s=\"http://lca.jrc.it/ILCD/Source\" xmlns:u=\"http://lca.jrc.it/ILCD/UnitGroup\" name=\"C4\" scenario=\"0\"/>", "<ns11:modules xmlns:ns11=\"http://openlca.org/epd_ilcd\" xmlns=\"http://lca.jrc.it/ILCD/Process\" xmlns:c=\"http://lca.jrc.it/ILCD/Contact\" xmlns:common=\"http://lca.jrc.it/ILCD/Common\" xmlns:epd=\"http://www.iai.kit.edu/EPD/2013\" xmlns:epd2=\"http://www.indata.network/EPD/2019\" xmlns:f=\"http://lca.jrc.it/ILCD/Flow\" xmlns:fp=\"http://lca.jrc.it/ILCD/FlowProperty\" xmlns:m=\"http://lca.jrc.it/ILCD/LCIAMethod\" xmlns:ns9=\"http://www.okworx.com/ILCD/Extensions/2018/Profile\" xmlns:s=\"http://lca.jrc.it/ILCD/Source\" xmlns:u=\"http://lca.jrc.it/ILCD/UnitGroup\" name=\"C4\" scenario=\"Thermische Verwertung\"/>", "<ns11:modules xmlns:ns11=\"http://openlca.org/epd_ilcd\" xmlns=\"http://lca.jrc.it/ILCD/Process\" xmlns:c=\"http://lca.jrc.it/ILCD/Contact\" xmlns:common=\"http://lca.jrc.it/ILCD/Common\" xmlns:epd=\"http://www.iai.kit.edu/EPD/2013\" xmlns:epd2=\"http://www.indata.network/EPD/2019\" xmlns:f=\"http://lca.jrc.it/ILCD/Flow\" xmlns:fp=\"http://lca.jrc.it/ILCD/FlowProperty\" xmlns:m=\"http://lca.jrc.it/ILCD/LCIAMethod\" xmlns:ns9=\"http://www.okworx.com/ILCD/Extensions/2018/Profile\" xmlns:s=\"http://lca.jrc.it/ILCD/Source\" xmlns:u=\"http://lca.jrc.it/ILCD/UnitGroup\" name=\"D\" scenario=\"0\"/>", "<ns11:modules xmlns:ns11=\"http://openlca.org/epd_ilcd\" xmlns=\"http://lca.jrc.it/ILCD/Process\" xmlns:c=\"http://lca.jrc.it/ILCD/Contact\" xmlns:common=\"http://lca.jrc.it/ILCD/Common\" xmlns:epd=\"http://www.iai.kit.edu/EPD/2013\" xmlns:epd2=\"http://www.indata.network/EPD/2019\" xmlns:f=\"http://lca.jrc.it/ILCD/Flow\" xmlns:fp=\"http://lca.jrc.it/ILCD/FlowProperty\" xmlns:m=\"http://lca.jrc.it/ILCD/LCIAMethod\" xmlns:ns9=\"http://www.okworx.com/ILCD/Extensions/2018/Profile\" xmlns:s=\"http://lca.jrc.it/ILCD/Source\" xmlns:u=\"http://lca.jrc.it/ILCD/UnitGroup\" name=\"D\" scenario=\"Thermische Verwertung\"/>"]}}, "quantitativeReference": {"referenceToReferenceFlow": [1], "type": "Reference flow(s)"}, "time": {"referenceYear": 2025, "dataSetValidUntil": 2030, "timeRepresentativenessDescription": [{"value": " Die erhobenen Vordergrunddaten beziehen sich auf das Jahr 2022. ", "lang": "de"}, {"value": "The foreground data collected refers to the year 2022.", "lang": "en"}], "other": {"anies": [{"name": "publicationDateOfEPD", "value": 1749340800000}]}}, "geography": {"locationOfOperationSupplyOrProduction": {"descriptionOfRestrictions": [{"value": "Die Auslieferung des Produkts erfolgt ausschließlich mittels LKW. Die Transportdistanz ist vom tatsächlichen Einsatzort abhängig, wobei aktuell Deutschland und Österreich, sowie die Schweiz, Großbritannien und Benelux-Staaten relevante Absatzmärkte darstellen. Die mittlere Transportdistanz beträgt 267 km.", "lang": "de"}, {"value": "The product is delivered exclusively by truck. The transport distance depends on the actual place of use, with Germany, Austria, Switzerland, Great Britain and the Benelux countries currently representing relevant sales markets. The average transport distance is 267 km.", "lang": "en"}], "location": "DE"}}, "technology": {"technologyDescriptionAndIncludedProcesses": [{"value": "Bei dem Dämmstoff handelt es sich um Hobelspäne, die beim Hobeln verschiedener Weichholzarten aus nahegelegenen regionalen Sägewerken entstehen. Verwendet werden vor allem Fichte in reiner Sortierung, eventuell kleine Restmengen von Tanne und Kiefer. Als Flammschutzmittel und gegen Schimmelpilz werden die Späne mit Molke und Soda imprägniert.", "lang": "de"}, {"value": "The insulation material consists of wood shavings produced during the planing of various types of softwood from nearby regional sawmills. Pure spruce is mainly used, with small amounts of fir and pine possibly also being used. The shavings are impregnated with whey and soda as a flame retardant and to prevent mould growth.", "lang": "en"}], "technologicalApplicability": [{"value": "Die HOIZ - Hobelspandämmung wird als Wärme- und Schalldämmstoff für Dächer, Decken und Wände als nicht belastbare Hohlraumdämmung im Holzbau eingesetzt. Generell können jedoch alle Hohlräume von Bauteilen (auch Stahlkonstruktionen) damit gedämmt bzw. akustisch gedämmt werden.\r\nDer Dämmstoff wird jedoch nur werksintern in Fertigteile verbaut und nicht als „reiner“ Dämmstoff separat ausgeliefert.\r\n", "lang": "de"}, {"value": "HOIZ - wood shaving insulation is used as thermal and sound insulation for roofs, ceilings and walls as non-load-bearing cavity insulation in timber construction. In general all cavities in building components (including steel structures) could be insulated or acoustically insulated with it. \r\nHowever, the insulation material is only installed in prefabricated parts in-house and is not delivered separately as a ‘pure’ insulation material.", "lang": "en"}]}}, "modellingAndValidation": {"LCIMethodAndAllocation": {"typeOfDataSet": "EPD", "referenceToLCAMethodDetails": [{"shortDescription": [{"value": "PKR Bau EPD GmbH PKR-Code: 2.22.5 Version 12.0 Stand 20.09.2023 \"Dämmstoffe aus nachwachsenden Rohstoffen\"", "lang": "de"}], "type": "source data set", "refObjectId": "7d5585c9-0fd2-4b95-bf48-722f260e46b0", "version": "00.00.000"}], "other": {"anies": [{"name": "subType", "value": "specific dataset"}]}}, "dataSourcesTreatmentAndRepresentativeness": {"referenceToDataSource": [{"shortDescription": [{"value": "GaBi database (general)", "lang": "en"}], "type": "source data set", "refObjectId": "28d74cc0-db8b-4d7e-bc44-5f6d56ce0c4a", "version": "00.03.002"}, {"shortDescription": [{"value": "Sphera MLC (fka GaBi) Databases Edition 2024", "lang": "en"}], "type": "source data set", "refObjectId": "7443b962-0446-4d69-8aa7-8055a6b1614a", "version": "00.01.000"}, {"shortDescription": [{"value": "Software: LCA for Experts (Version 10.9.0.31)", "lang": "de"}], "type": "source data set", "refObjectId": "b9605bc1-84c0-449f-95ef-c6a816b5d757", "version": "00.00.001"}], "useAdviceForDataSet": [{"value": "Anwendung im Gebäude sinnvoll. Grundsätzlich ist eine Gegenüberstellung oder die Bewertung von EPD Daten nur möglich, wenn alle zu vergleichenden Datensätze nach EN 15804 erstellt wurden und die produktspezifischen Leistungsmerkmale berücksichtigt werden.\r\nAnwendung ausschließlich in Baufritz Systemwänden.\r\n", "lang": "de"}], "other": {"anies": [{"name": "referenceToOriginalEPD", "value": {"shortDescription": {"value": "Bau EPD GmbH EPD GABI Baufritz 2025-01", "defaultValue": "Bau EPD GmbH EPD GABI Baufritz 2025-01", "lstrings": [{"lang": "de", "value": "Bau EPD GmbH EPD GABI Baufritz 2025-01"}]}, "version": {"version": 1, "majorVersion": 0, "minorVersion": 0, "subMinorVersion": 1, "zero": false, "versionString": "00.00.001"}, "uri": "http://openlca.org/ilcd/resource/sources/ed07cc37-ac91-43e7-9629-c0e795e338c5", "href": "http://openlca.org/ilcd/resource/sources/ed07cc37-ac91-43e7-9629-c0e795e338c5", "type": "source data set", "uuid": {"uuid": "ecb30682-e9ba-41f6-abde-ddd91e109e1d"}, "refObjectId": "ecb30682-e9ba-41f6-abde-ddd91e109e1d", "versionAsString": "00.00.001", "resourceURLs": ["https://oekobaudat.de/OEKOBAU.DAT/resource/sources/ecb30682-e9ba-41f6-abde-ddd91e109e1d/BAU-EPD-Baufritz-2025-1-GaBi-Hoiz-20250608-Webseite.pdf?version=00.00.001"]}}]}}, "validation": {"review": [{"reviewDetails": [{"value": "keine", "lang": "de"}], "referenceToNameOfReviewerAndInstitution": [{"shortDescription": [{"value": "Bau EPD GmbH", "lang": "de"}, {"value": "Bau EPD GmbH", "lang": "en"}], "type": "contact data set", "refObjectId": "42398bec-0af8-444e-9221-d40be4c4f553", "version": "00.00.007", "uri": "http://openlca.org/ilcd/resource/contacts/42398bec-0af8-444e-9221-d40be4c4f553"}], "type": "Accredited third party review"}]}, "complianceDeclarations": {"compliance": [{"referenceToComplianceSystem": {"shortDescription": [{"value": "ISO 14025", "lang": "en"}], "type": "source data set", "refObjectId": "4f2eb655-6e44-4874-a95a-e28f5442cd4d", "version": "00.00.001"}}, {"referenceToComplianceSystem": {"shortDescription": [{"value": "EN 15804+A2 (EF 3.1)", "lang": "de"}, {"value": "EN 15804+A2 (EF 3.1)", "lang": "en"}], "type": "source data set", "refObjectId": "d4aa3ec7-b1d7-4a4a-a6cb-37af88dcc902", "version": "00.01.000"}}]}}, "administrativeInformation": {"commissionerAndGoal": {"referenceToCommissioner": [{"shortDescription": [{"value": "Baufritz GmbH & Co KG", "lang": "de"}], "type": "contact data set", "refObjectId": "5d49884b-5657-4e9a-84b4-aa6504423144", "version": "00.00.002"}]}, "dataGenerator": {"referenceToPersonOrEntityGeneratingTheDataSet": [{"shortDescription": [{"value": "Verifier Daxner, Therese", "lang": "de"}], "type": "contact data set", "refObjectId": "2c60822c-6304-4b81-84e1-3cf3aaabfa77", "version": "00.00.003"}, {"shortDescription": [{"value": "Verifier Gschösser, Florian", "lang": "de"}], "type": "contact data set", "refObjectId": "da875289-3cae-4746-91a3-e7b476932b81", "version": "00.00.005"}]}, "dataEntryBy": {"timeStamp": 1753187982409, "referenceToDataSetFormat": [{"shortDescription": [{"value": "EPD Data Format Extensions v1.2", "lang": "en"}, {"value": "EPD-Datenformaterweiterungen v1.2", "lang": "de"}], "type": "source data set", "refObjectId": "a29449fd-aa2f-4de8-b5d7-4b06b43c6fde", "version": "00.01.000"}, {"shortDescription": [{"value": "ILCD format", "lang": "en"}], "type": "source data set", "refObjectId": "a97a0155-0234-4b87-b4ce-a45da52f2a40", "version": "01.00.000", "uri": "http://lca.jrc.ec.europa.eu/lcainfohub/sample_data/ilcd/sources/ILCD_Format_a97a0155-0234-4b87-b4ce-a45da52f2a40_01.00.000.xml"}], "referenceToPersonOrEntityEnteringTheData": {"shortDescription": [{"value": "Bau EPD GmbH", "lang": "de"}, {"value": "Bau EPD GmbH", "lang": "en"}], "type": "contact data set", "refObjectId": "42398bec-0af8-444e-9221-d40be4c4f553", "version": "00.00.007", "uri": "http://openlca.org/ilcd/resource/contacts/42398bec-0af8-444e-9221-d40be4c4f553"}}, "publicationAndOwnership": {"dataSetVersion": "00.00.010", "referenceToPrecedingDataSetVersion": [{"shortDescription": [{"value": "Baufritz GaBi HOIZ Hobelspandämmung", "lang": "de"}], "otherAttributes": {"{http://greendelta.com/epd-editor}referenceYear": "2018", "{http://greendelta.com/epd-editor}database": "GaBi"}, "type": "process data set", "refObjectId": "2d22c5e2-ffd0-4f70-903d-a5d553f439dd", "version": "00.00.022"}], "referenceToRegistrationAuthority": {"shortDescription": [{"value": "Bau EPD GmbH", "lang": "de"}, {"value": "Bau EPD GmbH", "lang": "en"}], "type": "contact data set", "refObjectId": "42398bec-0af8-444e-9221-d40be4c4f553", "version": "00.00.007", "uri": "http://openlca.org/ilcd/resource/contacts/42398bec-0af8-444e-9221-d40be4c4f553"}, "registrationNumber": "BAU-EPD-Baufritz-2025-1-GaBi-Hoiz ", "referenceToOwnershipOfDataSet": {"shortDescription": [{"value": "Bau EPD GmbH", "lang": "de"}, {"value": "Bau EPD GmbH", "lang": "en"}], "type": "contact data set", "refObjectId": "42398bec-0af8-444e-9221-d40be4c4f553", "version": "00.00.007", "uri": "http://openlca.org/ilcd/resource/contacts/42398bec-0af8-444e-9221-d40be4c4f553"}, "copyright": true, "licenseType": "Free of charge for all users and uses", "accessRestrictions": [{"value": "keine", "lang": "de"}], "other": {"anies": [{"name": "referenceToPublisher", "value": {"shortDescription": [{"value": "Bau EPD GmbH", "lang": "de"}, {"value": "Bau EPD GmbH", "lang": "en"}], "type": "contact data set", "refObjectId": "42398bec-0af8-444e-9221-d40be4c4f553", "version": "00.00.007", "uri": "http://openlca.org/ilcd/resource/contacts/42398bec-0af8-444e-9221-d40be4c4f553"}}]}}}, "exchanges": {"exchange": [{"dataSetInternalID": 1, "referenceToFlowDataSet": {"shortDescription": [{"value": "Baufritz HOIZ Hobelspandämmung NA 2025", "lang": "de"}], "type": "flow data set", "refObjectId": "50d14dac-c400-48af-ab31-b5a2562231d1", "version": "00.00.001"}, "meanAmount": 1.0, "resultingAmount": 1.0, "referenceFlow": true, "resultingflowAmount": 1.0, "flowProperties": [{"name": [{"lang": "en", "value": "Volume"}, {"lang": "de", "value": "Volumen"}], "uuid": "93a60a56-a3c8-22da-a746-0800200c9a66", "referenceFlowProperty": true, "meanValue": 1.0, "referenceUnit": "m3", "unitGroupUUID": "cd950537-0a98-4044-9ba7-9f9a68d0a504"}, {"name": [{"lang": "en", "value": "Carbon content (biogenic)"}], "uuid": "62e503ce-544a-4599-b2ad-bcea15a7bf20", "meanValue": 30.33}, {"name": [{"lang": "de", "value": "Masse"}, {"lang": "en", "value": "Mass"}], "uuid": "93a60a56-a3c8-11da-a746-0800200b9a66", "meanValue": 1.0}, {"name": [{"lang": "en", "value": "Carbon content (biogenic) - packaging"}], "uuid": "262a541b-209e-44cc-a426-33bce30de7b1", "meanValue": 0.0}], "materialProperties": [{"name": "gross density", "value": "70.0", "unit": "kg/m^3", "unitDescription": "kilograms per cubic metre"}], "typeOfFlow": "Product flow", "classification": {"classHierarchy": "Dämmstoffe / Holzfasern", "name": "ilcd"}}, {"dataSetInternalID": 2, "referenceToFlowDataSet": {"shortDescription": [{"value": "Use of renewable primary energy (PERE)", "lang": "en"}, {"value": "Erneuerbare Primärenergie als Energieträger (PERE)", "lang": "de"}, {"value": "Uso de energía primaria renovable excluyendo los recursos de energía primaria renovable utilizada como materia prima (PERE)", "lang": "es"}], "type": "flow data set", "refObjectId": "20f32be5-0398-4288-9b6d-accddd195317", "version": "38.00.000", "uri": "../flows/20f32be5-0398-4288-9b6d-accddd195317.xml"}, "exchange direction": "INPUT", "meanAmount": 0.0, "other": {"anies": [{"value": "266.4067791857685", "module": "A1-A3"}, {"value": "2.68081810506299", "module": "A4"}, {"value": "0.0", "module": "A5"}, {"value": "0.0", "module": "B1"}, {"value": "0.0", "module": "B2"}, {"value": "0.0", "module": "B3"}, {"value": "0.0", "module": "B4"}, {"value": "0.0", "module": "B5"}, {"value": "0.0", "module": "B6"}, {"value": "0.0", "module": "B7"}, {"value": "0.0", "module": "C1", "scenario": "Thermische Verwertung"}, {"value": "1.00405172474269", "module": "C2", "scenario": "Thermische Verwertung"}, {"value": "1064.889261874963", "module": "C3", "scenario": "Thermische Verwertung"}, {"value": "0.0", "module": "C4", "scenario": "Thermische Verwertung"}, {"value": "-187.938006616063", "module": "D", "scenario": "Thermische Verwertung"}, {"name": "referenceToUnitGroupDataSet", "value": {"shortDescription": [{"value": "MJ", "lang": "en"}], "type": "unit group data set", "refObjectId": "93a60a57-a3c8-11da-a746-0800200c9a66", "version": "03.00.000", "uri": "../unitgroups/93a60a57-a3c8-11da-a746-0800200c9a66.xml"}}]}, "flowProperties": [], "typeOfFlow": "Other flow", "classification": {"classHierarchy": "Quantities", "name": "GaBiCategories"}}, {"dataSetInternalID": 3, "referenceToFlowDataSet": {"shortDescription": [{"value": "Use of renewable primary energy resources used as raw materials (PERM)", "lang": "en"}, {"value": "Erneuerbare Primärenergie zur stofflichen Nutzung (PERM)", "lang": "de"}, {"value": "Uso de energía primaria renovable utilizada como materia prima (PERM)", "lang": "es"}], "type": "flow data set", "refObjectId": "fb3ec0de-548d-4508-aea5-00b73bf6f702", "version": "38.00.000", "uri": "../flows/fb3ec0de-548d-4508-aea5-00b73bf6f702.xml"}, "exchange direction": "INPUT", "meanAmount": 0.0, "other": {"anies": [{"value": "1057.5", "module": "A1-A3"}, {"value": "0.0", "module": "A4"}, {"value": "0.0", "module": "A5"}, {"value": "0.0", "module": "B1"}, {"value": "0.0", "module": "B2"}, {"value": "0.0", "module": "B3"}, {"value": "0.0", "module": "B4"}, {"value": "0.0", "module": "B5"}, {"value": "0.0", "module": "B6"}, {"value": "0.0", "module": "B7"}, {"value": "0.0", "module": "C1", "scenario": "Thermische Verwertung"}, {"value": "0.0", "module": "C2", "scenario": "Thermische Verwertung"}, {"value": "-1057.5", "module": "C3", "scenario": "Thermische Verwertung"}, {"value": "0.0", "module": "C4", "scenario": "Thermische Verwertung"}, {"value": "0.0", "module": "D", "scenario": "Thermische Verwertung"}, {"name": "referenceToUnitGroupDataSet", "value": {"shortDescription": [{"value": "MJ", "lang": "en"}], "type": "unit group data set", "refObjectId": "93a60a57-a3c8-11da-a746-0800200c9a66", "version": "03.00.000", "uri": "../unitgroups/93a60a57-a3c8-11da-a746-0800200c9a66.xml"}}]}, "flowProperties": [], "typeOfFlow": "Other flow", "classification": {"classHierarchy": "Quantities", "name": "GaBiCategories"}}, {"dataSetInternalID": 4, "referenceToFlowDataSet": {"shortDescription": [{"value": "Total use of renewable primary energy resources (PERT)", "lang": "en"}, {"value": "Total erneuerbare Primärenergie (PERT)", "lang": "de"}, {"value": "Uso total de la energía primaria renovable (energía primaria y recursos de energía primaria renovable utilizada como materia prima) (PERT)", "lang": "es"}], "type": "flow data set", "refObjectId": "53f97275-fa8a-4cdd-9024-65936002acd0", "version": "30.00.000", "uri": "../flows/53f97275-fa8a-4cdd-9024-65936002acd0.xml"}, "exchange direction": "INPUT", "meanAmount": 0.0, "other": {"anies": [{"value": "1323.9067791857685", "module": "A1-A3"}, {"value": "2.68081810506299", "module": "A4"}, {"value": "0.0", "module": "A5"}, {"value": "0.0", "module": "B1"}, {"value": "0.0", "module": "B2"}, {"value": "0.0", "module": "B3"}, {"value": "0.0", "module": "B4"}, {"value": "0.0", "module": "B5"}, {"value": "0.0", "module": "B6"}, {"value": "0.0", "module": "B7"}, {"value": "0.0", "module": "C1", "scenario": "Thermische Verwertung"}, {"value": "1.00405172474269", "module": "C2", "scenario": "Thermische Verwertung"}, {"value": "7.38926187496304", "module": "C3", "scenario": "Thermische Verwertung"}, {"value": "0.0", "module": "C4", "scenario": "Thermische Verwertung"}, {"value": "-187.938006616063", "module": "D", "scenario": "Thermische Verwertung"}, {"name": "referenceToUnitGroupDataSet", "value": {"shortDescription": [{"value": "MJ", "lang": "en"}], "type": "unit group data set", "refObjectId": "93a60a57-a3c8-11da-a746-0800200c9a66", "version": "03.00.000", "uri": "../unitgroups/93a60a57-a3c8-11da-a746-0800200c9a66.xml"}}]}, "flowProperties": [], "typeOfFlow": "Other flow", "classification": {"classHierarchy": "Größen / Umweltliche Größen / EPD EN 15804 / LCI Indikatoren", "name": "GaBiCategories"}}, {"dataSetInternalID": 5, "referenceToFlowDataSet": {"shortDescription": [{"value": "Use of non renewable primary energy (PENRE)", "lang": "en"}, {"value": "Nicht-erneuerbare Primärenergie als Energieträger (PENRE)", "lang": "de"}, {"value": "Uso de energía primaria no renovable, excluyendo los recursos de energía primaria no renovable utilizada como materia prima (PENRE)", "lang": "es"}], "type": "flow data set", "refObjectId": "ac857178-2b45-46ec-892a-a9a4332f0372", "version": "38.00.000", "uri": "../flows/ac857178-2b45-46ec-892a-a9a4332f0372.xml"}, "exchange direction": "INPUT", "meanAmount": 0.0, "other": {"anies": [{"value": "179.85325700485217", "module": "A1-A3"}, {"value": "24.2240794121061", "module": "A4"}, {"value": "0.0", "module": "A5"}, {"value": "0.0", "module": "B1"}, {"value": "0.0", "module": "B2"}, {"value": "0.0", "module": "B3"}, {"value": "0.0", "module": "B4"}, {"value": "0.0", "module": "B5"}, {"value": "0.0", "module": "B6"}, {"value": "0.0", "module": "B7"}, {"value": "0.0", "module": "C1", "scenario": "Thermische Verwertung"}, {"value": "9.07268891839177", "module": "C2", "scenario": "Thermische Verwertung"}, {"value": "26.1076252385281", "module": "C3", "scenario": "Thermische Verwertung"}, {"value": "0.0", "module": "C4", "scenario": "Thermische Verwertung"}, {"value": "-556.119725691822", "module": "D", "scenario": "Thermische Verwertung"}, {"name": "referenceToUnitGroupDataSet", "value": {"shortDescription": [{"value": "MJ", "lang": "en"}], "type": "unit group data set", "refObjectId": "93a60a57-a3c8-11da-a746-0800200c9a66", "version": "03.00.000", "uri": "../unitgroups/93a60a57-a3c8-11da-a746-0800200c9a66.xml"}}]}, "flowProperties": [], "typeOfFlow": "Other flow", "classification": {"classHierarchy": "Quantities", "name": "GaBiCategories"}}, {"dataSetInternalID": 6, "referenceToFlowDataSet": {"shortDescription": [{"value": "Use of non renewable primary energy resources used as raw materials (PENRM)", "lang": "en"}, {"value": "Nicht-erneuerbare Primärenergie zur stofflichen Nutzung (PENRM)", "lang": "de"}, {"value": "Uso de la energía primaria no renovable utilizada como materia prima (PENRM)", "lang": "es"}], "type": "flow data set", "refObjectId": "1421caa0-679d-4bf4-b282-0eb850ccae27", "version": "38.00.000", "uri": "../flows/1421caa0-679d-4bf4-b282-0eb850ccae27.xml"}, "exchange direction": "INPUT", "meanAmount": 0.0, "other": {"anies": [{"value": "0.0", "module": "A1-A3"}, {"value": "0.0", "module": "A4"}, {"value": "0.0", "module": "A5"}, {"value": "0.0", "module": "B1"}, {"value": "0.0", "module": "B2"}, {"value": "0.0", "module": "B3"}, {"value": "0.0", "module": "B4"}, {"value": "0.0", "module": "B5"}, {"value": "0.0", "module": "B6"}, {"value": "0.0", "module": "B7"}, {"value": "0.0", "module": "C1", "scenario": "Thermische Verwertung"}, {"value": "0.0", "module": "C2", "scenario": "Thermische Verwertung"}, {"value": "0.0", "module": "C3", "scenario": "Thermische Verwertung"}, {"value": "0.0", "module": "C4", "scenario": "Thermische Verwertung"}, {"value": "0.0", "module": "D", "scenario": "Thermische Verwertung"}, {"name": "referenceToUnitGroupDataSet", "value": {"shortDescription": [{"value": "MJ", "lang": "en"}], "type": "unit group data set", "refObjectId": "93a60a57-a3c8-11da-a746-0800200c9a66", "version": "03.00.000", "uri": "../unitgroups/93a60a57-a3c8-11da-a746-0800200c9a66.xml"}}]}, "flowProperties": [], "typeOfFlow": "Other flow", "classification": {"classHierarchy": "Quantities", "name": "GaBiCategories"}}, {"dataSetInternalID": 7, "referenceToFlowDataSet": {"shortDescription": [{"value": "Total use of non-renewable primary energy resources (PENRT)", "lang": "en"}, {"value": "Total nicht erneuerbare Primärenergie (PENRT)", "lang": "de"}, {"value": "Uso total de la energía primaria no renovable (energía primaria y recursos de energía primaria renovable utilizada como materia prima) (PENRT)", "lang": "es"}], "type": "flow data set", "refObjectId": "06159210-646b-4c8d-8583-da9b3b95a6c1", "version": "30.00.000", "uri": "../flows/06159210-646b-4c8d-8583-da9b3b95a6c1.xml"}, "exchange direction": "INPUT", "meanAmount": 0.0, "other": {"anies": [{"value": "179.85325700485217", "module": "A1-A3"}, {"value": "24.2240794121061", "module": "A4"}, {"value": "0.0", "module": "A5"}, {"value": "0.0", "module": "B1"}, {"value": "0.0", "module": "B2"}, {"value": "0.0", "module": "B3"}, {"value": "0.0", "module": "B4"}, {"value": "0.0", "module": "B5"}, {"value": "0.0", "module": "B6"}, {"value": "0.0", "module": "B7"}, {"value": "0.0", "module": "C1", "scenario": "Thermische Verwertung"}, {"value": "9.07268891839177", "module": "C2", "scenario": "Thermische Verwertung"}, {"value": "26.1076252385281", "module": "C3", "scenario": "Thermische Verwertung"}, {"value": "0.0", "module": "C4", "scenario": "Thermische Verwertung"}, {"value": "-556.119725691822", "module": "D", "scenario": "Thermische Verwertung"}, {"name": "referenceToUnitGroupDataSet", "value": {"shortDescription": [{"value": "MJ", "lang": "en"}], "type": "unit group data set", "refObjectId": "93a60a57-a3c8-11da-a746-0800200c9a66", "version": "03.00.000", "uri": "../unitgroups/93a60a57-a3c8-11da-a746-0800200c9a66.xml"}}]}, "flowProperties": [], "typeOfFlow": "Other flow", "classification": {"classHierarchy": "Größen / Umweltliche Größen / EPD EN 15804 / LCI Indikatoren", "name": "GaBiCategories"}}, {"dataSetInternalID": 8, "referenceToFlowDataSet": {"shortDescription": [{"value": "Use of secondary material (SM)", "lang": "en"}, {"value": "Einsatz von Sekundärstoffen (SM)", "lang": "de"}, {"value": "Uso de materiales secundarios (SM)", "lang": "es"}], "type": "flow data set", "refObjectId": "c6a1f35f-2d09-4f54-8dfb-97e502e1ce92", "version": "30.00.000", "uri": "../flows/c6a1f35f-2d09-4f54-8dfb-97e502e1ce92.xml"}, "exchange direction": "INPUT", "meanAmount": 0.0, "other": {"anies": [{"value": "0.0", "module": "A1-A3"}, {"value": "0.0", "module": "A4"}, {"value": "0.0", "module": "A5"}, {"value": "0.0", "module": "B1"}, {"value": "0.0", "module": "B2"}, {"value": "0.0", "module": "B3"}, {"value": "0.0", "module": "B4"}, {"value": "0.0", "module": "B5"}, {"value": "0.0", "module": "B6"}, {"value": "0.0", "module": "B7"}, {"value": "0.0", "module": "C1", "scenario": "Thermische Verwertung"}, {"value": "0.0", "module": "C2", "scenario": "Thermische Verwertung"}, {"value": "0.0", "module": "C3", "scenario": "Thermische Verwertung"}, {"value": "0.0", "module": "C4", "scenario": "Thermische Verwertung"}, {"value": "0.0", "module": "D", "scenario": "Thermische Verwertung"}, {"name": "referenceToUnitGroupDataSet", "value": {"shortDescription": [{"value": "kg", "lang": "en"}], "type": "unit group data set", "refObjectId": "ad38d542-3fe9-439d-9b95-2f5f7752acaf", "version": "30.00.000", "uri": "../unitgroups/ad38d542-3fe9-439d-9b95-2f5f7752acaf.xml"}}]}, "flowProperties": [], "typeOfFlow": "Other flow", "classification": {"classHierarchy": "Größen / Umweltliche Größen / EPD EN 15804 / LCI Indikatoren", "name": "GaBiCategories"}}, {"dataSetInternalID": 9, "referenceToFlowDataSet": {"shortDescription": [{"value": "Use of renewable secondary fuels (RSF)", "lang": "en"}, {"value": "Erneuerbare Sekundärbrennstoffe (RSF)", "lang": "de"}, {"value": "Uso de combustibles secundarios renovables (RSF)", "lang": "es"}], "type": "flow data set", "refObjectId": "64333088-a55f-4aa2-9a31-c10b07816787", "version": "30.00.000", "uri": "../flows/64333088-a55f-4aa2-9a31-c10b07816787.xml"}, "exchange direction": "INPUT", "meanAmount": 0.0, "other": {"anies": [{"value": "0.0", "module": "A1-A3"}, {"value": "0.0", "module": "A4"}, {"value": "0.0", "module": "A5"}, {"value": "0.0", "module": "B1"}, {"value": "0.0", "module": "B2"}, {"value": "0.0", "module": "B3"}, {"value": "0.0", "module": "B4"}, {"value": "0.0", "module": "B5"}, {"value": "0.0", "module": "B6"}, {"value": "0.0", "module": "B7"}, {"value": "0.0", "module": "C1", "scenario": "Thermische Verwertung"}, {"value": "0.0", "module": "C2", "scenario": "Thermische Verwertung"}, {"value": "0.0", "module": "C3", "scenario": "Thermische Verwertung"}, {"value": "0.0", "module": "C4", "scenario": "Thermische Verwertung"}, {"value": "0.0", "module": "D", "scenario": "Thermische Verwertung"}, {"name": "referenceToUnitGroupDataSet", "value": {"shortDescription": [{"value": "MJ", "lang": "en"}], "type": "unit group data set", "refObjectId": "93a60a57-a3c8-11da-a746-0800200c9a66", "version": "03.00.000", "uri": "../unitgroups/93a60a57-a3c8-11da-a746-0800200c9a66.xml"}}]}, "flowProperties": [], "typeOfFlow": "Other flow", "classification": {"classHierarchy": "Größen / Umweltliche Größen / EPD EN 15804 / LCI Indikatoren", "name": "GaBiCategories"}}, {"dataSetInternalID": 10, "referenceToFlowDataSet": {"shortDescription": [{"value": "Use of non renewable secondary fuels (NRSF)", "lang": "en"}, {"value": "Nicht erneuerbare Sekundärbrennstoffe (NRSF)", "lang": "de"}, {"value": "Uso de combustibles secundarios no renovables (NRSF)", "lang": "es"}], "type": "flow data set", "refObjectId": "89def144-d39a-4287-b86f-efde453ddcb2", "version": "30.00.000", "uri": "../flows/89def144-d39a-4287-b86f-efde453ddcb2.xml"}, "exchange direction": "INPUT", "meanAmount": 0.0, "other": {"anies": [{"value": "0.0", "module": "A1-A3"}, {"value": "0.0", "module": "A4"}, {"value": "0.0", "module": "A5"}, {"value": "0.0", "module": "B1"}, {"value": "0.0", "module": "B2"}, {"value": "0.0", "module": "B3"}, {"value": "0.0", "module": "B4"}, {"value": "0.0", "module": "B5"}, {"value": "0.0", "module": "B6"}, {"value": "0.0", "module": "B7"}, {"value": "0.0", "module": "C1", "scenario": "Thermische Verwertung"}, {"value": "0.0", "module": "C2", "scenario": "Thermische Verwertung"}, {"value": "0.0", "module": "C3", "scenario": "Thermische Verwertung"}, {"value": "0.0", "module": "C4", "scenario": "Thermische Verwertung"}, {"value": "0.0", "module": "D", "scenario": "Thermische Verwertung"}, {"name": "referenceToUnitGroupDataSet", "value": {"shortDescription": [{"value": "MJ", "lang": "en"}], "type": "unit group data set", "refObjectId": "93a60a57-a3c8-11da-a746-0800200c9a66", "version": "03.00.000", "uri": "../unitgroups/93a60a57-a3c8-11da-a746-0800200c9a66.xml"}}]}, "flowProperties": [], "typeOfFlow": "Other flow", "classification": {"classHierarchy": "Größen / Umweltliche Größen / EPD EN 15804 / LCI Indikatoren", "name": "GaBiCategories"}}, {"dataSetInternalID": 11, "referenceToFlowDataSet": {"shortDescription": [{"value": "Use of net fresh water (FW)", "lang": "en"}, {"value": "Einsatz von Süßwasserressourcen (FW)", "lang": "de"}, {"value": "Uso neto de recursos de agua dulce (FW)", "lang": "es"}], "type": "flow data set", "refObjectId": "3cf952c8-f3a4-461d-8c96-96456ca62246", "version": "30.00.000", "uri": "../flows/3cf952c8-f3a4-461d-8c96-96456ca62246.xml"}, "exchange direction": "INPUT", "meanAmount": 0.0, "other": {"anies": [{"value": "0.07197521735251827", "module": "A1-A3"}, {"value": "0.00250446329922588", "module": "A4"}, {"value": "0.0", "module": "A5"}, {"value": "0.0", "module": "B1"}, {"value": "0.0", "module": "B2"}, {"value": "0.0", "module": "B3"}, {"value": "0.0", "module": "B4"}, {"value": "0.0", "module": "B5"}, {"value": "0.0", "module": "B6"}, {"value": "0.0", "module": "B7"}, {"value": "0.0", "module": "C1", "scenario": "Thermische Verwertung"}, {"value": "9.38001235665106E-4", "module": "C2", "scenario": "Thermische Verwertung"}, {"value": "0.276761408840894", "module": "C3", "scenario": "Thermische Verwertung"}, {"value": "0.0", "module": "C4", "scenario": "Thermische Verwertung"}, {"value": "-0.144307127842666", "module": "D", "scenario": "Thermische Verwertung"}, {"name": "referenceToUnitGroupDataSet", "value": {"shortDescription": [{"value": "m3", "lang": "en"}], "type": "unit group data set", "refObjectId": "cd950537-0a98-4044-9ba7-9f9a68d0a504", "version": "30.00.000", "uri": "../unitgroups/cd950537-0a98-4044-9ba7-9f9a68d0a504.xml"}}]}, "flowProperties": [], "typeOfFlow": "Other flow", "classification": {"classHierarchy": "Größen / Umweltliche Größen / EPD EN 15804 / LCI Indikatoren", "name": "GaBiCategories"}}, {"dataSetInternalID": 12, "referenceToFlowDataSet": {"shortDescription": [{"value": "Hazardous waste disposed (HWD)", "lang": "en"}, {"value": "Gefährlicher Abfall zur Deponie (HWD)", "lang": "de"}, {"value": "Residuos peligrosos eliminados (HWD)", "lang": "es"}], "type": "flow data set", "refObjectId": "430f9e0f-59b2-46a0-8e0d-55e0e84948fc", "version": "30.00.000", "uri": "../flows/430f9e0f-59b2-46a0-8e0d-55e0e84948fc.xml"}, "exchange direction": "OUTPUT", "meanAmount": 0.0, "other": {"anies": [{"value": "1.8519073397442432E-4", "module": "A1-A3"}, {"value": "1.17932758345343E-9", "module": "A4"}, {"value": "0.0", "module": "A5"}, {"value": "0.0", "module": "B1"}, {"value": "0.0", "module": "B2"}, {"value": "0.0", "module": "B3"}, {"value": "0.0", "module": "B4"}, {"value": "0.0", "module": "B5"}, {"value": "0.0", "module": "B6"}, {"value": "0.0", "module": "B7"}, {"value": "0.0", "module": "C1", "scenario": "Thermische Verwertung"}, {"value": "4.41695724139862E-10", "module": "C2", "scenario": "Thermische Verwertung"}, {"value": "1.53602521090035E-8", "module": "C3", "scenario": "Thermische Verwertung"}, {"value": "0.0", "module": "C4", "scenario": "Thermische Verwertung"}, {"value": "-3.80175147324729E-7", "module": "D", "scenario": "Thermische Verwertung"}, {"name": "referenceToUnitGroupDataSet", "value": {"shortDescription": [{"value": "kg", "lang": "en"}], "type": "unit group data set", "refObjectId": "ad38d542-3fe9-439d-9b95-2f5f7752acaf", "version": "30.00.000", "uri": "../unitgroups/ad38d542-3fe9-439d-9b95-2f5f7752acaf.xml"}}]}, "flowProperties": [], "typeOfFlow": "Other flow", "classification": {"classHierarchy": "Größen / Umweltliche Größen / EPD EN 15804 / LCI Indikatoren", "name": "GaBiCategories"}}, {"dataSetInternalID": 13, "referenceToFlowDataSet": {"shortDescription": [{"value": "Non-hazardous waste disposed (NHWD)", "lang": "en"}, {"value": "Entsorgter nicht gefährlicher Abfall (NHWD)", "lang": "de"}, {"value": "Residuos no peligrosos eliminados (NHWD)", "lang": "es"}], "type": "flow data set", "refObjectId": "b29ef66b-e286-4afa-949f-62f1a7b4d7fa", "version": "30.00.000", "uri": "../flows/b29ef66b-e286-4afa-949f-62f1a7b4d7fa.xml"}, "exchange direction": "OUTPUT", "meanAmount": 0.0, "other": {"anies": [{"value": "2.6809935273835555", "module": "A1-A3"}, {"value": "0.00409574558900485", "module": "A4"}, {"value": "0.0", "module": "A5"}, {"value": "0.0", "module": "B1"}, {"value": "0.0", "module": "B2"}, {"value": "0.0", "module": "B3"}, {"value": "0.0", "module": "B4"}, {"value": "0.0", "module": "B5"}, {"value": "0.0", "module": "B6"}, {"value": "0.0", "module": "B7"}, {"value": "0.0", "module": "C1", "scenario": "Thermische Verwertung"}, {"value": "0.00153398711198683", "module": "C2", "scenario": "Thermische Verwertung"}, {"value": "2.10410574855312", "module": "C3", "scenario": "Thermische Verwertung"}, {"value": "0.0", "module": "C4", "scenario": "Thermische Verwertung"}, {"value": "-0.291128394592827", "module": "D", "scenario": "Thermische Verwertung"}, {"name": "referenceToUnitGroupDataSet", "value": {"shortDescription": [{"value": "kg", "lang": "en"}], "type": "unit group data set", "refObjectId": "ad38d542-3fe9-439d-9b95-2f5f7752acaf", "version": "30.00.000", "uri": "../unitgroups/ad38d542-3fe9-439d-9b95-2f5f7752acaf.xml"}}]}, "flowProperties": [], "typeOfFlow": "Other flow", "classification": {"classHierarchy": "Größen / Umweltliche Größen / EPD EN 15804 / LCI Indikatoren", "name": "GaBiCategories"}}, {"dataSetInternalID": 14, "referenceToFlowDataSet": {"shortDescription": [{"value": "Radioactive waste disposed (RWD)", "lang": "en"}, {"value": "Entsorgter radioaktiver Abfall (RWD)", "lang": "de"}, {"value": "Residuos radiactivos eliminados (RWD)", "lang": "es"}], "type": "flow data set", "refObjectId": "3449546e-52ad-4b39-b809-9fb77cea8ff6", "version": "30.00.000", "uri": "../flows/3449546e-52ad-4b39-b809-9fb77cea8ff6.xml"}, "exchange direction": "OUTPUT", "meanAmount": 0.0, "other": {"anies": [{"value": "0.002490958851129434", "module": "A1-A3"}, {"value": "3.85566984844185E-5", "module": "A4"}, {"value": "0.0", "module": "A5"}, {"value": "0.0", "module": "B1"}, {"value": "0.0", "module": "B2"}, {"value": "0.0", "module": "B3"}, {"value": "0.0", "module": "B4"}, {"value": "0.0", "module": "B5"}, {"value": "0.0", "module": "B6"}, {"value": "0.0", "module": "B7"}, {"value": "0.0", "module": "C1", "scenario": "Thermische Verwertung"}, {"value": "1.44407110428534E-5", "module": "C2", "scenario": "Thermische Verwertung"}, {"value": "0.00140769609225029", "module": "C3", "scenario": "Thermische Verwertung"}, {"value": "0.0", "module": "C4", "scenario": "Thermische Verwertung"}, {"value": "-0.0415351719030932", "module": "D", "scenario": "Thermische Verwertung"}, {"name": "referenceToUnitGroupDataSet", "value": {"shortDescription": [{"value": "kg", "lang": "en"}], "type": "unit group data set", "refObjectId": "ad38d542-3fe9-439d-9b95-2f5f7752acaf", "version": "30.00.000", "uri": "../unitgroups/ad38d542-3fe9-439d-9b95-2f5f7752acaf.xml"}}]}, "flowProperties": [], "typeOfFlow": "Other flow", "classification": {"classHierarchy": "Größen / Umweltliche Größen / EPD EN 15804 / LCI Indikatoren", "name": "GaBiCategories"}}, {"dataSetInternalID": 15, "referenceToFlowDataSet": {"shortDescription": [{"value": "Components for re-use (CRU)", "lang": "en"}, {"value": "Komponenten für die Wiederverwendung (CRU)", "lang": "de"}, {"value": "Componentes para su reutilización (CRU)", "lang": "es"}], "type": "flow data set", "refObjectId": "a2b32f97-3fc7-4af2-b209-525bc6426f33", "version": "30.00.000", "uri": "../flows/a2b32f97-3fc7-4af2-b209-525bc6426f33.xml"}, "exchange direction": "OUTPUT", "meanAmount": 0.0, "other": {"anies": [{"value": "0.0", "module": "A1-A3"}, {"value": "0.0", "module": "A4"}, {"value": "0.0", "module": "A5"}, {"value": "0.0", "module": "B1"}, {"value": "0.0", "module": "B2"}, {"value": "0.0", "module": "B3"}, {"value": "0.0", "module": "B4"}, {"value": "0.0", "module": "B5"}, {"value": "0.0", "module": "B6"}, {"value": "0.0", "module": "B7"}, {"value": "0.0", "module": "C1", "scenario": "Thermische Verwertung"}, {"value": "0.0", "module": "C2", "scenario": "Thermische Verwertung"}, {"value": "0.0", "module": "C3", "scenario": "Thermische Verwertung"}, {"value": "0.0", "module": "C4", "scenario": "Thermische Verwertung"}, {"value": "0.0", "module": "D", "scenario": "Thermische Verwertung"}, {"name": "referenceToUnitGroupDataSet", "value": {"shortDescription": [{"value": "kg", "lang": "en"}], "type": "unit group data set", "refObjectId": "ad38d542-3fe9-439d-9b95-2f5f7752acaf", "version": "30.00.000", "uri": "../unitgroups/ad38d542-3fe9-439d-9b95-2f5f7752acaf.xml"}}]}, "flowProperties": [], "typeOfFlow": "Other flow", "classification": {"classHierarchy": "Größen / Umweltliche Größen / EPD EN 15804 / LCI Indikatoren", "name": "GaBiCategories"}}, {"dataSetInternalID": 16, "referenceToFlowDataSet": {"shortDescription": [{"value": "Materials for recycling (MFR)", "lang": "en"}, {"value": "Stoffe zum Recycling (MFR)", "lang": "de"}, {"value": "Materiales para el reciclaje (MFR)", "lang": "es"}], "type": "flow data set", "refObjectId": "d7fe48a5-4103-49c8-9aae-b0b5dfdbd6ae", "version": "30.00.000", "uri": "../flows/d7fe48a5-4103-49c8-9aae-b0b5dfdbd6ae.xml"}, "exchange direction": "OUTPUT", "meanAmount": 0.0, "other": {"anies": [{"value": "0.0", "module": "A1-A3"}, {"value": "0.0", "module": "A4"}, {"value": "0.0", "module": "A5"}, {"value": "0.0", "module": "B1"}, {"value": "0.0", "module": "B2"}, {"value": "0.0", "module": "B3"}, {"value": "0.0", "module": "B4"}, {"value": "0.0", "module": "B5"}, {"value": "0.0", "module": "B6"}, {"value": "0.0", "module": "B7"}, {"value": "0.0", "module": "C1", "scenario": "Thermische Verwertung"}, {"value": "0.0", "module": "C2", "scenario": "Thermische Verwertung"}, {"value": "0.0", "module": "C3", "scenario": "Thermische Verwertung"}, {"value": "0.0", "module": "C4", "scenario": "Thermische Verwertung"}, {"value": "0.0", "module": "D", "scenario": "Thermische Verwertung"}, {"name": "referenceToUnitGroupDataSet", "value": {"shortDescription": [{"value": "kg", "lang": "en"}], "type": "unit group data set", "refObjectId": "ad38d542-3fe9-439d-9b95-2f5f7752acaf", "version": "30.00.000", "uri": "../unitgroups/ad38d542-3fe9-439d-9b95-2f5f7752acaf.xml"}}]}, "flowProperties": [], "typeOfFlow": "Other flow", "classification": {"classHierarchy": "Größen / Umweltliche Größen / EPD EN 15804 / LCI Indikatoren", "name": "GaBiCategories"}}, {"dataSetInternalID": 17, "referenceToFlowDataSet": {"shortDescription": [{"value": "Materials for energy recovery (MER)", "lang": "en"}, {"value": "Stoffe für die Energierückgewinnung (MER)", "lang": "de"}, {"value": "Materiales para valorización energética (recuperación de energía) (MER)", "lang": "es"}], "type": "flow data set", "refObjectId": "59a9181c-3aaf-46ee-8b13-2b3723b6e447", "version": "30.00.000", "uri": "../flows/59a9181c-3aaf-46ee-8b13-2b3723b6e447.xml"}, "exchange direction": "OUTPUT", "meanAmount": 0.0, "other": {"anies": [{"value": "0.0", "module": "A1-A3"}, {"value": "0.0", "module": "A4"}, {"value": "0.0", "module": "A5"}, {"value": "0.0", "module": "B1"}, {"value": "0.0", "module": "B2"}, {"value": "0.0", "module": "B3"}, {"value": "0.0", "module": "B4"}, {"value": "0.0", "module": "B5"}, {"value": "0.0", "module": "B6"}, {"value": "0.0", "module": "B7"}, {"value": "0.0", "module": "C1", "scenario": "Thermische Verwertung"}, {"value": "0.0", "module": "C2", "scenario": "Thermische Verwertung"}, {"value": "0.0", "module": "C3", "scenario": "Thermische Verwertung"}, {"value": "0.0", "module": "C4", "scenario": "Thermische Verwertung"}, {"value": "0.0", "module": "D", "scenario": "Thermische Verwertung"}, {"name": "referenceToUnitGroupDataSet", "value": {"shortDescription": [{"value": "kg", "lang": "en"}], "type": "unit group data set", "refObjectId": "ad38d542-3fe9-439d-9b95-2f5f7752acaf", "version": "30.00.000", "uri": "../unitgroups/ad38d542-3fe9-439d-9b95-2f5f7752acaf.xml"}}]}, "flowProperties": [], "typeOfFlow": "Other flow", "classification": {"classHierarchy": "Größen / Umweltliche Größen / EPD EN 15804 / LCI Indikatoren", "name": "GaBiCategories"}}, {"dataSetInternalID": 18, "referenceToFlowDataSet": {"shortDescription": [{"value": "Exported electrical energy (EEE)", "lang": "en"}, {"value": "Exportierte elektrische Energie (EEE)", "lang": "de"}, {"value": "Energía exportada electrica (EEE)", "lang": "es"}], "type": "flow data set", "refObjectId": "4da0c987-2b76-40d6-9e9e-82a017aaaf29", "version": "30.00.000", "uri": "../flows/4da0c987-2b76-40d6-9e9e-82a017aaaf29.xml"}, "exchange direction": "OUTPUT", "meanAmount": 0.0, "other": {"anies": [{"value": "0.0", "module": "A1-A3"}, {"value": "0.0", "module": "A4"}, {"value": "0.0", "module": "A5"}, {"value": "0.0", "module": "B1"}, {"value": "0.0", "module": "B2"}, {"value": "0.0", "module": "B3"}, {"value": "0.0", "module": "B4"}, {"value": "0.0", "module": "B5"}, {"value": "0.0", "module": "B6"}, {"value": "0.0", "module": "B7"}, {"value": "0.0", "module": "C1", "scenario": "Thermische Verwertung"}, {"value": "0.0", "module": "C2", "scenario": "Thermische Verwertung"}, {"value": "268.368171330605", "module": "C3", "scenario": "Thermische Verwertung"}, {"value": "0.0", "module": "C4", "scenario": "Thermische Verwertung"}, {"value": "0.0", "module": "D", "scenario": "Thermische Verwertung"}, {"name": "referenceToUnitGroupDataSet", "value": {"shortDescription": [{"value": "MJ", "lang": "en"}], "type": "unit group data set", "refObjectId": "93a60a57-a3c8-11da-a746-0800200c9a66", "version": "03.00.000", "uri": "../unitgroups/93a60a57-a3c8-11da-a746-0800200c9a66.xml"}}]}, "flowProperties": [], "typeOfFlow": "Other flow", "classification": {"classHierarchy": "Größen / Umweltliche Größen / EPD EN 15804 / LCI Indikatoren", "name": "GaBiCategories"}}, {"dataSetInternalID": 19, "referenceToFlowDataSet": {"shortDescription": [{"value": "Exported thermal energy (EET)", "lang": "en"}, {"value": "Exportierte thermische Energie (EET)", "lang": "de"}, {"value": "Energía exportada termal (EET)", "lang": "es"}], "type": "flow data set", "refObjectId": "98daf38a-7a79-46d3-9a37-2b7bd0955810", "version": "30.00.000", "uri": "../flows/98daf38a-7a79-46d3-9a37-2b7bd0955810.xml"}, "exchange direction": "OUTPUT", "meanAmount": 0.0, "other": {"anies": [{"value": "0.0", "module": "A1-A3"}, {"value": "0.0", "module": "A4"}, {"value": "0.0", "module": "A5"}, {"value": "0.0", "module": "B1"}, {"value": "0.0", "module": "B2"}, {"value": "0.0", "module": "B3"}, {"value": "0.0", "module": "B4"}, {"value": "0.0", "module": "B5"}, {"value": "0.0", "module": "B6"}, {"value": "0.0", "module": "B7"}, {"value": "0.0", "module": "C1", "scenario": "Thermische Verwertung"}, {"value": "0.0", "module": "C2", "scenario": "Thermische Verwertung"}, {"value": "148.912903778076", "module": "C3", "scenario": "Thermische Verwertung"}, {"value": "0.0", "module": "C4", "scenario": "Thermische Verwertung"}, {"value": "0.0", "module": "D", "scenario": "Thermische Verwertung"}, {"name": "referenceToUnitGroupDataSet", "value": {"shortDescription": [{"value": "MJ", "lang": "en"}], "type": "unit group data set", "refObjectId": "93a60a57-a3c8-11da-a746-0800200c9a66", "version": "03.00.000", "uri": "../unitgroups/93a60a57-a3c8-11da-a746-0800200c9a66.xml"}}]}, "flowProperties": [], "typeOfFlow": "Other flow", "classification": {"classHierarchy": "Größen / Umweltliche Größen / EPD EN 15804 / LCI Indikatoren", "name": "GaBiCategories"}}]}, "LCIAResults": {"LCIAResult": [{"referenceToLCIAMethodDataSet": {"shortDescription": [{"value": "Global Warming Potential - total (GWP-total)", "lang": "en"}, {"value": "Globales Erwärmungspotenzial - total (GWP-total)", "lang": "de"}], "type": "LCIA method data set", "refObjectId": "a7ea142a-9749-11ed-a8fc-0242ac120002", "version": "04.00.017", "uri": "../lciamethods/a7ea142a-9749-11ed-a8fc-0242ac120002.xml"}, "meanAmount": 0.0, "other": {"anies": [{"value": "-96.44079114837942", "module": "A1-A3"}, {"value": "1.8867278026614829", "module": "A4"}, {"value": "0.0", "module": "A5"}, {"value": "0.0", "module": "B1"}, {"value": "0.0", "module": "B2"}, {"value": "0.0", "module": "B3"}, {"value": "0.0", "module": "B4"}, {"value": "0.0", "module": "B5"}, {"value": "0.0", "module": "B6"}, {"value": "0.0", "module": "B7"}, {"value": "0.0", "module": "C1", "scenario": "Thermische Verwertung"}, {"value": "0.706639626464973", "module": "C2", "scenario": "Thermische Verwertung"}, {"value": "113.03165208570603", "module": "C3", "scenario": "Thermische Verwertung"}, {"value": "0.0", "module": "C4", "scenario": "Thermische Verwertung"}, {"value": "-31.24456563381161", "module": "D", "scenario": "Thermische Verwertung"}, {"name": "referenceToUnitGroupDataSet", "value": {"shortDescription": [{"value": "kg CO2-eq.", "lang": "en"}], "type": "unit group data set", "refObjectId": "1ebf3012-d0db-4de2-aefd-ef30cedb0be1", "version": "30.00.000", "uri": "../unitgroups/1ebf3012-d0db-4de2-aefd-ef30cedb0be1.xml"}}]}}, {"referenceToLCIAMethodDataSet": {"shortDescription": [{"value": "Global Warming Potential - fossil fuels (GWP-fossil)", "lang": "en"}, {"value": "Globales Erwärmungspotenzial - fossil (GWP-fossil)", "lang": "de"}], "type": "LCIA method data set", "refObjectId": "a7ea19c0-9749-11ed-a8fc-0242ac120002", "version": "01.00.009", "uri": "../lciamethods/a7ea19c0-9749-11ed-a8fc-0242ac120002.xml"}, "meanAmount": 0.0, "other": {"anies": [{"value": "13.843710518583297", "module": "A1-A3"}, {"value": "1.84068685667914", "module": "A4"}, {"value": "0.0", "module": "A5"}, {"value": "0.0", "module": "B1"}, {"value": "0.0", "module": "B2"}, {"value": "0.0", "module": "B3"}, {"value": "0.0", "module": "B4"}, {"value": "0.0", "module": "B5"}, {"value": "0.0", "module": "B6"}, {"value": "0.0", "module": "B7"}, {"value": "0.0", "module": "C1", "scenario": "Thermische Verwertung"}, {"value": "0.689395826471586", "module": "C2", "scenario": "Thermische Verwertung"}, {"value": "1.82135640149071", "module": "C3", "scenario": "Thermische Verwertung"}, {"value": "0.0", "module": "C4", "scenario": "Thermische Verwertung"}, {"value": "-31.1059208735083", "module": "D", "scenario": "Thermische Verwertung"}, {"name": "referenceToUnitGroupDataSet", "value": {"shortDescription": [{"value": "kg CO2-eq.", "lang": "en"}], "type": "unit group data set", "refObjectId": "1ebf3012-d0db-4de2-aefd-ef30cedb0be1", "version": "30.00.000", "uri": "../unitgroups/1ebf3012-d0db-4de2-aefd-ef30cedb0be1.xml"}}]}}, {"referenceToLCIAMethodDataSet": {"shortDescription": [{"value": "Global Warming Potential - biogenic (GWP-biogenic)", "lang": "en"}, {"value": "Globales Erwärmungspotenzial - biogen (GWP-biogenic)", "lang": "de"}], "type": "LCIA method data set", "refObjectId": "a7ea186c-9749-11ed-a8fc-0242ac120002", "version": "01.00.006", "uri": "../lciamethods/a7ea186c-9749-11ed-a8fc-0242ac120002.xml"}, "meanAmount": 0.0, "other": {"anies": [{"value": "-111.20926666666665", "module": "A1-A3"}, {"value": "0.0105552911510072", "module": "A4"}, {"value": "0.0", "module": "A5"}, {"value": "0.0", "module": "B1"}, {"value": "0.0", "module": "B2"}, {"value": "0.0", "module": "B3"}, {"value": "0.0", "module": "B4"}, {"value": "0.0", "module": "B5"}, {"value": "0.0", "module": "B6"}, {"value": "0.0", "module": "B7"}, {"value": "0.0", "module": "C1", "scenario": "Thermische Verwertung"}, {"value": "0.00395329256592038", "module": "C2", "scenario": "Thermische Verwertung"}, {"value": "111.20926666666665", "module": "C3", "scenario": "Thermische Verwertung"}, {"value": "0.0", "module": "C4", "scenario": "Thermische Verwertung"}, {"value": "-0.135804735694501", "module": "D", "scenario": "Thermische Verwertung"}, {"name": "referenceToUnitGroupDataSet", "value": {"shortDescription": [{"value": "kg CO2-eq.", "lang": "en"}], "type": "unit group data set", "refObjectId": "1ebf3012-d0db-4de2-aefd-ef30cedb0be1", "version": "30.00.000", "uri": "../unitgroups/1ebf3012-d0db-4de2-aefd-ef30cedb0be1.xml"}}]}}, {"referenceToLCIAMethodDataSet": {"shortDescription": [{"value": "Global Warming Potential - land use and land use change (GWP-luluc)", "lang": "en"}, {"value": "Globales Erwärmungspotenzial - luluc (GWP-luluc)", "lang": "de"}], "type": "LCIA method data set", "refObjectId": "a7ea1ae2-9749-11ed-a8fc-0242ac120002", "version": "01.00.006", "uri": "../lciamethods/a7ea1ae2-9749-11ed-a8fc-0242ac120002.xml"}, "meanAmount": 0.0, "other": {"anies": [{"value": "0.9247649997039408", "module": "A1-A3"}, {"value": "0.0354856548313358", "module": "A4"}, {"value": "0.0", "module": "A5"}, {"value": "0.0", "module": "B1"}, {"value": "0.0", "module": "B2"}, {"value": "0.0", "module": "B3"}, {"value": "0.0", "module": "B4"}, {"value": "0.0", "module": "B5"}, {"value": "0.0", "module": "B6"}, {"value": "0.0", "module": "B7"}, {"value": "0.0", "module": "C1", "scenario": "Thermische Verwertung"}, {"value": "0.0132905074274666", "module": "C2", "scenario": "Thermische Verwertung"}, {"value": "0.00102901754867493", "module": "C3", "scenario": "Thermische Verwertung"}, {"value": "0.0", "module": "C4", "scenario": "Thermische Verwertung"}, {"value": "-0.00284002460881134", "module": "D", "scenario": "Thermische Verwertung"}, {"name": "referenceToUnitGroupDataSet", "value": {"shortDescription": [{"value": "kg CO2-eq.", "lang": "en"}], "type": "unit group data set", "refObjectId": "1ebf3012-d0db-4de2-aefd-ef30cedb0be1", "version": "30.00.000", "uri": "../unitgroups/1ebf3012-d0db-4de2-aefd-ef30cedb0be1.xml"}}]}}, {"referenceToLCIAMethodDataSet": {"shortDescription": [{"value": "Depletion potential of the stratospheric ozone layer (ODP)", "lang": "en"}, {"value": "Abbaupotenzial der stratosphärischen Ozonschicht (ODP)", "lang": "de"}], "type": "LCIA method data set", "refObjectId": "b5c629d6-def3-11e6-bf01-fe55135034f3", "version": "02.00.013", "uri": "../lciamethods/b5c629d6-def3-11e6-bf01-fe55135034f3.xml"}, "meanAmount": 0.0, "other": {"anies": [{"value": "6.209601408646499E-8", "module": "A1-A3"}, {"value": "5.82585189048259E-13", "module": "A4"}, {"value": "0.0", "module": "A5"}, {"value": "0.0", "module": "B1"}, {"value": "0.0", "module": "B2"}, {"value": "0.0", "module": "B3"}, {"value": "0.0", "module": "B4"}, {"value": "0.0", "module": "B5"}, {"value": "0.0", "module": "B6"}, {"value": "0.0", "module": "B7"}, {"value": "0.0", "module": "C1", "scenario": "Thermische Verwertung"}, {"value": "2.18196700018074E-13", "module": "C2", "scenario": "Thermische Verwertung"}, {"value": "1.18404544517552E-11", "module": "C3", "scenario": "Thermische Verwertung"}, {"value": "0.0", "module": "C4", "scenario": "Thermische Verwertung"}, {"value": "-2.80747914447445E-10", "module": "D", "scenario": "Thermische Verwertung"}, {"name": "referenceToUnitGroupDataSet", "value": {"shortDescription": [{"value": "kg CFC-11-eq.", "lang": "en"}], "type": "unit group data set", "refObjectId": "d9e957c9-7309-4474-bf3a-7777df6c4e5b", "version": "25.00.000", "uri": "../unitgroups/d9e957c9-7309-4474-bf3a-7777df6c4e5b.xml"}}]}}, {"referenceToLCIAMethodDataSet": {"shortDescription": [{"value": "Acidification potential, Accumulated Exceedance (AP)", "lang": "en"}, {"value": "Versauerungspotenzial, kumulierte Überschreitung (AP)", "lang": "de"}], "type": "LCIA method data set", "refObjectId": "b5c611c6-def3-11e6-bf01-fe55135034f3", "version": "01.03.010", "uri": "../lciamethods/b5c611c6-def3-11e6-bf01-fe55135034f3.xml"}, "meanAmount": 0.0, "other": {"anies": [{"value": "0.08989876822859802", "module": "A1-A3"}, {"value": "0.00257080589893899", "module": "A4"}, {"value": "0.0", "module": "A5"}, {"value": "0.0", "module": "B1"}, {"value": "0.0", "module": "B2"}, {"value": "0.0", "module": "B3"}, {"value": "0.0", "module": "B4"}, {"value": "0.0", "module": "B5"}, {"value": "0.0", "module": "B6"}, {"value": "0.0", "module": "B7"}, {"value": "0.0", "module": "C1", "scenario": "Thermische Verwertung"}, {"value": "9.62848651288009E-4", "module": "C2", "scenario": "Thermische Verwertung"}, {"value": "0.0177369476853953", "module": "C3", "scenario": "Thermische Verwertung"}, {"value": "0.0", "module": "C4", "scenario": "Thermische Verwertung"}, {"value": "-0.0328794012061881", "module": "D", "scenario": "Thermische Verwertung"}, {"name": "referenceToUnitGroupDataSet", "value": {"shortDescription": [{"value": "mol H+-eq.", "lang": "en"}], "type": "unit group data set", "refObjectId": "42e089ac-92bf-4bf2-8ca1-5fc40d18f2ed", "version": "00.01.000", "uri": "../unitgroups/42e089ac-92bf-4bf2-8ca1-5fc40d18f2ed.xml"}}]}}, {"referenceToLCIAMethodDataSet": {"shortDescription": [{"value": "Eutrophication potential - freshwater (EP-freshwater)", "lang": "en"}, {"value": "Eutrophierungspotenzial - Süßwasser (EP-freshwater)", "lang": "de"}], "type": "LCIA method data set", "refObjectId": "b53ec18f-7377-4ad3-86eb-cc3f4f276b2b", "version": "01.00.011", "uri": "../lciamethods/b53ec18f-7377-4ad3-86eb-cc3f4f276b2b.xml"}, "meanAmount": 0.0, "other": {"anies": [{"value": "0.0011196972569700381", "module": "A1-A3"}, {"value": "5.02400909610274E-6", "module": "A4"}, {"value": "0.0", "module": "A5"}, {"value": "0.0", "module": "B1"}, {"value": "0.0", "module": "B2"}, {"value": "0.0", "module": "B3"}, {"value": "0.0", "module": "B4"}, {"value": "0.0", "module": "B5"}, {"value": "0.0", "module": "B6"}, {"value": "0.0", "module": "B7"}, {"value": "0.0", "module": "C1", "scenario": "Thermische Verwertung"}, {"value": "1.88165134685496E-6", "module": "C2", "scenario": "Thermische Verwertung"}, {"value": "3.04245280437394E-6", "module": "C3", "scenario": "Thermische Verwertung"}, {"value": "0.0", "module": "C4", "scenario": "Thermische Verwertung"}, {"value": "-5.23598365247789E-5", "module": "D", "scenario": "Thermische Verwertung"}, {"name": "referenceToUnitGroupDataSet", "value": {"shortDescription": [{"value": "kg P-eq.", "lang": "en"}], "type": "unit group data set", "refObjectId": "0429039d-a61d-4590-ba67-aa4a20a810a1", "version": "30.00.000", "uri": "../unitgroups/0429039d-a61d-4590-ba67-aa4a20a810a1.xml"}}]}}, {"referenceToLCIAMethodDataSet": {"shortDescription": [{"value": "Eutrophication potential - marine (EP-marine)", "lang": "en"}, {"value": "Eutrophierungspotenzial - Salzwasser (EP-marine)", "lang": "de"}], "type": "LCIA method data set", "refObjectId": "b5c619fa-def3-11e6-bf01-fe55135034f3", "version": "02.00.011", "uri": "../lciamethods/b5c619fa-def3-11e6-bf01-fe55135034f3.xml"}, "meanAmount": 0.0, "other": {"anies": [{"value": "0.035050156180576095", "module": "A1-A3"}, {"value": "9.50113849708235E-4", "module": "A4"}, {"value": "0.0", "module": "A5"}, {"value": "0.0", "module": "B1"}, {"value": "0.0", "module": "B2"}, {"value": "0.0", "module": "B3"}, {"value": "0.0", "module": "B4"}, {"value": "0.0", "module": "B5"}, {"value": "0.0", "module": "B6"}, {"value": "0.0", "module": "B7"}, {"value": "0.0", "module": "C1", "scenario": "Thermische Verwertung"}, {"value": "3.55847883785856E-4", "module": "C2", "scenario": "Thermische Verwertung"}, {"value": "0.005193467236315", "module": "C3", "scenario": "Thermische Verwertung"}, {"value": "0.0", "module": "C4", "scenario": "Thermische Verwertung"}, {"value": "-0.010005711028052", "module": "D", "scenario": "Thermische Verwertung"}, {"name": "referenceToUnitGroupDataSet", "value": {"shortDescription": [{"value": "kg N-eq.", "lang": "en"}], "type": "unit group data set", "refObjectId": "d05bb823-ecdf-4686-8c40-bf1d9257859f", "version": "00.00.003", "uri": "../unitgroups/d05bb823-ecdf-4686-8c40-bf1d9257859f.xml"}}]}}, {"referenceToLCIAMethodDataSet": {"shortDescription": [{"value": "Eutrophication potential - terrestrial (EP-terrestrial)", "lang": "en"}, {"value": "Eutrophierungspotenzial - Land (EP-terrestrial)", "lang": "de"}], "type": "LCIA method data set", "refObjectId": "b5c614d2-def3-11e6-bf01-fe55135034f3", "version": "01.02.010", "uri": "../lciamethods/b5c614d2-def3-11e6-bf01-fe55135034f3.xml"}, "meanAmount": 0.0, "other": {"anies": [{"value": "0.3747484379399321", "module": "A1-A3"}, {"value": "0.0114591647751039", "module": "A4"}, {"value": "0.0", "module": "A5"}, {"value": "0.0", "module": "B1"}, {"value": "0.0", "module": "B2"}, {"value": "0.0", "module": "B3"}, {"value": "0.0", "module": "B4"}, {"value": "0.0", "module": "B5"}, {"value": "0.0", "module": "B6"}, {"value": "0.0", "module": "B7"}, {"value": "0.0", "module": "C1", "scenario": "Thermische Verwertung"}, {"value": "0.00429182201314752", "module": "C2", "scenario": "Thermische Verwertung"}, {"value": "0.0743781954093409", "module": "C3", "scenario": "Thermische Verwertung"}, {"value": "0.0", "module": "C4", "scenario": "Thermische Verwertung"}, {"value": "-0.107355104154753", "module": "D", "scenario": "Thermische Verwertung"}, {"name": "referenceToUnitGroupDataSet", "value": {"shortDescription": [{"value": "mol N-eq.", "lang": "en"}], "type": "unit group data set", "refObjectId": "71b4d617-0ec9-4d3f-b65e-e438940c2401", "version": "00.00.003", "uri": "../unitgroups/71b4d617-0ec9-4d3f-b65e-e438940c2401.xml"}}]}}, {"referenceToLCIAMethodDataSet": {"shortDescription": [{"value": "Photochemical Ozone Creation Potential (POCP)", "lang": "en"}, {"value": "Bildungspotenzial für troposphärisches Ozon (POCP)", "lang": "de"}], "type": "LCIA method data set", "refObjectId": "b5c610fe-def3-11e6-bf01-fe55135034f3", "version": "02.00.015", "uri": "../lciamethods/b5c610fe-def3-11e6-bf01-fe55135034f3.xml"}, "meanAmount": 0.0, "other": {"anies": [{"value": "0.04418529606695439", "module": "A1-A3"}, {"value": "0.00252835655438749", "module": "A4"}, {"value": "0.0", "module": "A5"}, {"value": "0.0", "module": "B1"}, {"value": "0.0", "module": "B2"}, {"value": "0.0", "module": "B3"}, {"value": "0.0", "module": "B4"}, {"value": "0.0", "module": "B5"}, {"value": "0.0", "module": "B6"}, {"value": "0.0", "module": "B7"}, {"value": "0.0", "module": "C1", "scenario": "Thermische Verwertung"}, {"value": "9.46950020369847E-4", "module": "C2", "scenario": "Thermische Verwertung"}, {"value": "0.0142977347402924", "module": "C3", "scenario": "Thermische Verwertung"}, {"value": "0.0", "module": "C4", "scenario": "Thermische Verwertung"}, {"value": "-0.0283150659292594", "module": "D", "scenario": "Thermische Verwertung"}, {"name": "referenceToUnitGroupDataSet", "value": {"shortDescription": [{"value": "kg NMVOC-eq.", "lang": "en"}], "type": "unit group data set", "refObjectId": "d27c25f8-fbc1-44c6-b47b-4adbae4199c6", "version": "00.00.003", "uri": "../unitgroups/d27c25f8-fbc1-44c6-b47b-4adbae4199c6.xml"}}]}}, {"referenceToLCIAMethodDataSet": {"shortDescription": [{"value": "Abiotic depletion potential - non-fossil resources (ADPE)", "lang": "en"}, {"value": "Potenzial für die Verknappung abiotischer Ressourcen – nicht fossile Ressourcen (ADPE)", "lang": "de"}], "type": "LCIA method data set", "refObjectId": "b2ad6494-c78d-11e6-9d9d-cec0c932ce01", "version": "01.00.011", "uri": "../lciamethods/b2ad6494-c78d-11e6-9d9d-cec0c932ce01.xml"}, "meanAmount": 0.0, "other": {"anies": [{"value": "2.7075978992940454E-5", "module": "A1-A3"}, {"value": "3.14029884728064E-7", "module": "A4"}, {"value": "0.0", "module": "A5"}, {"value": "0.0", "module": "B1"}, {"value": "0.0", "module": "B2"}, {"value": "0.0", "module": "B3"}, {"value": "0.0", "module": "B4"}, {"value": "0.0", "module": "B5"}, {"value": "0.0", "module": "B6"}, {"value": "0.0", "module": "B7"}, {"value": "0.0", "module": "C1", "scenario": "Thermische Verwertung"}, {"value": "1.17614189036728E-7", "module": "C2", "scenario": "Thermische Verwertung"}, {"value": "1.25924754751842E-7", "module": "C3", "scenario": "Thermische Verwertung"}, {"value": "0.0", "module": "C4", "scenario": "Thermische Verwertung"}, {"value": "-2.72586963865728E-6", "module": "D", "scenario": "Thermische Verwertung"}, {"name": "referenceToUnitGroupDataSet", "value": {"shortDescription": [{"value": "kg Sb-eq.", "lang": "en"}], "type": "unit group data set", "refObjectId": "54ccd2d9-a32a-4fc2-923d-f2c8c93e89d4", "version": "30.00.000", "uri": "../unitgroups/54ccd2d9-a32a-4fc2-923d-f2c8c93e89d4.xml"}}]}}, {"referenceToLCIAMethodDataSet": {"shortDescription": [{"value": "Abiotic depletion potential - fossil resources (ADPF)", "lang": "en"}, {"value": "Potenzial für die Verknappung abiotischer Ressourcen – fossile Brennstoffe (ADPF)", "lang": "de"}], "type": "LCIA method data set", "refObjectId": "b2ad6110-c78d-11e6-9d9d-cec0c932ce01", "version": "01.00.011", "uri": "../lciamethods/b2ad6110-c78d-11e6-9d9d-cec0c932ce01.xml"}, "meanAmount": 0.0, "other": {"anies": [{"value": "179.85325700485217", "module": "A1-A3"}, {"value": "24.224079412106", "module": "A4"}, {"value": "0.0", "module": "A5"}, {"value": "0.0", "module": "B1"}, {"value": "0.0", "module": "B2"}, {"value": "0.0", "module": "B3"}, {"value": "0.0", "module": "B4"}, {"value": "0.0", "module": "B5"}, {"value": "0.0", "module": "B6"}, {"value": "0.0", "module": "B7"}, {"value": "0.0", "module": "C1", "scenario": "Thermische Verwertung"}, {"value": "9.07268891839176", "module": "C2", "scenario": "Thermische Verwertung"}, {"value": "26.1076252385278", "module": "C3", "scenario": "Thermische Verwertung"}, {"value": "0.0", "module": "C4", "scenario": "Thermische Verwertung"}, {"value": "-556.119725691813", "module": "D", "scenario": "Thermische Verwertung"}, {"name": "referenceToUnitGroupDataSet", "value": {"shortDescription": [{"value": "MJ", "lang": "en"}], "type": "unit group data set", "refObjectId": "93a60a57-a3c8-11da-a746-0800200c9a66", "version": "03.00.000", "uri": "../unitgroups/93a60a57-a3c8-11da-a746-0800200c9a66.xml"}}]}}, {"referenceToLCIAMethodDataSet": {"shortDescription": [{"value": "Water (user) deprivation potential (WDP)", "lang": "en"}, {"value": "Wasser-Entzugspotenzial (Benutzer) (WDP)", "lang": "de"}], "type": "LCIA method data set", "refObjectId": "b2ad66ce-c78d-11e6-9d9d-cec0c932ce01", "version": "03.00.015", "uri": "../lciamethods/b2ad66ce-c78d-11e6-9d9d-cec0c932ce01.xml"}, "meanAmount": 0.0, "other": {"anies": [{"value": "14.024601525199465", "module": "A1-A3"}, {"value": "0.0132233092656244", "module": "A4"}, {"value": "0.0", "module": "A5"}, {"value": "0.0", "module": "B1"}, {"value": "0.0", "module": "B2"}, {"value": "0.0", "module": "B3"}, {"value": "0.0", "module": "B4"}, {"value": "0.0", "module": "B5"}, {"value": "0.0", "module": "B6"}, {"value": "0.0", "module": "B7"}, {"value": "0.0", "module": "C1", "scenario": "Thermische Verwertung"}, {"value": "0.00495255028675073", "module": "C2", "scenario": "Thermische Verwertung"}, {"value": "11.7701828895827", "module": "C3", "scenario": "Thermische Verwertung"}, {"value": "0.0", "module": "C4", "scenario": "Thermische Verwertung"}, {"value": "-3.43873699135577", "module": "D", "scenario": "Thermische Verwertung"}, {"name": "referenceToUnitGroupDataSet", "value": {"shortDescription": [{"value": "m3 world eq. deprived", "lang": "en"}], "type": "unit group data set", "refObjectId": "6ae2df01-888e-46c8-b17d-49fa3869b476", "version": "00.00.003", "uri": "../unitgroups/6ae2df01-888e-46c8-b17d-49fa3869b476.xml"}}]}}, {"referenceToLCIAMethodDataSet": {"shortDescription": [{"value": "Potential incidence of disease due to PM emissions (PM)", "lang": "en"}, {"value": "Potenzielles Auftreten von Krankheiten aufgrund von Feinstaubemissionen (PM)", "lang": "de"}], "type": "LCIA method data set", "refObjectId": "b5c602c6-def3-11e6-bf01-fe55135034f3", "version": "02.00.012", "uri": "../lciamethods/b5c602c6-def3-11e6-bf01-fe55135034f3.xml"}, "meanAmount": 0.0, "other": {"anies": [{"value": "2.8005344993042797E-6", "module": "A1-A3"}, {"value": "2.39549197602803E-8", "module": "A4"}, {"value": "0.0", "module": "A5"}, {"value": "0.0", "module": "B1"}, {"value": "0.0", "module": "B2"}, {"value": "0.0", "module": "B3"}, {"value": "0.0", "module": "B4"}, {"value": "0.0", "module": "B5"}, {"value": "0.0", "module": "B6"}, {"value": "0.0", "module": "B7"}, {"value": "0.0", "module": "C1", "scenario": "Thermische Verwertung"}, {"value": "8.97188006003006E-9", "module": "C2", "scenario": "Thermische Verwertung"}, {"value": "1.1854828903165E-7", "module": "C3", "scenario": "Thermische Verwertung"}, {"value": "0.0", "module": "C4", "scenario": "Thermische Verwertung"}, {"value": "-2.69641144587121E-7", "module": "D", "scenario": "Thermische Verwertung"}, {"name": "referenceToUnitGroupDataSet", "value": {"shortDescription": [{"value": "Disease incidence", "lang": "en"}], "type": "unit group data set", "refObjectId": "3883559b-648f-4afc-8ba2-0bd24f3affa3", "version": "00.00.003", "uri": "../unitgroups/3883559b-648f-4afc-8ba2-0bd24f3affa3.xml"}}]}}, {"referenceToLCIAMethodDataSet": {"shortDescription": [{"value": "Potential Human exposure efficiency relative to U235 (IRP)", "lang": "en"}, {"value": "Potenzielle Wirkung durch Exposition des Menschen mit U235 (IRP)", "lang": "de"}], "type": "LCIA method data set", "refObjectId": "b5c632be-def3-11e6-bf01-fe55135034f3", "version": "01.00.012", "uri": "../lciamethods/b5c632be-def3-11e6-bf01-fe55135034f3.xml"}, "meanAmount": 0.0, "other": {"anies": [{"value": "0.46576953671692733", "module": "A1-A3"}, {"value": "0.00406757408011561", "module": "A4"}, {"value": "0.0", "module": "A5"}, {"value": "0.0", "module": "B1"}, {"value": "0.0", "module": "B2"}, {"value": "0.0", "module": "B3"}, {"value": "0.0", "module": "B4"}, {"value": "0.0", "module": "B5"}, {"value": "0.0", "module": "B6"}, {"value": "0.0", "module": "B7"}, {"value": "0.0", "module": "C1", "scenario": "Thermische Verwertung"}, {"value": "0.00152343598506202", "module": "C2", "scenario": "Thermische Verwertung"}, {"value": "0.223220836317137", "module": "C3", "scenario": "Thermische Verwertung"}, {"value": "0.0", "module": "C4", "scenario": "Thermische Verwertung"}, {"value": "-6.83866974001864", "module": "D", "scenario": "Thermische Verwertung"}, {"name": "referenceToUnitGroupDataSet", "value": {"shortDescription": [{"value": "kgBq U235-eq.", "lang": "en"}], "type": "unit group data set", "refObjectId": "456b05bf-1415-44a9-9993-02452f554c09", "version": "00.00.003", "uri": "../unitgroups/456b05bf-1415-44a9-9993-02452f554c09.xml"}}]}}, {"referenceToLCIAMethodDataSet": {"shortDescription": [{"value": "Potential Comparative Toxic Unit for ecosystems (ETP-fw)", "lang": "en"}, {"value": "Potenzielle Toxizitätsvergleichseinheit für Ökosysteme (ETP-fw)", "lang": "de"}], "type": "LCIA method data set", "refObjectId": "05316e7a-b254-4bea-9cf0-6bf33eb5c630", "version": "01.00.003", "uri": "../lciamethods/05316e7a-b254-4bea-9cf0-6bf33eb5c630.xml"}, "meanAmount": 0.0, "other": {"anies": [{"value": "262.1393079624172", "module": "A1-A3"}, {"value": "18.7997973884015", "module": "A4"}, {"value": "0.0", "module": "A5"}, {"value": "0.0", "module": "B1"}, {"value": "0.0", "module": "B2"}, {"value": "0.0", "module": "B3"}, {"value": "0.0", "module": "B4"}, {"value": "0.0", "module": "B5"}, {"value": "0.0", "module": "B6"}, {"value": "0.0", "module": "B7"}, {"value": "0.0", "module": "C1", "scenario": "Thermische Verwertung"}, {"value": "7.04112261737883", "module": "C2", "scenario": "Thermische Verwertung"}, {"value": "11.2550064018763", "module": "C3", "scenario": "Thermische Verwertung"}, {"value": "0.0", "module": "C4", "scenario": "Thermische Verwertung"}, {"value": "-79.3896108022398", "module": "D", "scenario": "Thermische Verwertung"}, {"name": "referenceToUnitGroupDataSet", "value": {"shortDescription": [{"value": "CTUe", "lang": "en"}], "type": "unit group data set", "refObjectId": "aa959ded-f1eb-4efb-9c5c-2d60be36b3e6", "version": "00.00.003", "uri": "../unitgroups/aa959ded-f1eb-4efb-9c5c-2d60be36b3e6.xml"}}]}}, {"referenceToLCIAMethodDataSet": {"shortDescription": [{"value": "Potential Comparative Toxic Unit for humans - cancer effects (HTP-c)", "lang": "en"}, {"value": "Potenzielle Toxizitätsvergleichseinheit für den Menschen - kanzerogene Wirkung (HTP-c)", "lang": "de"}], "type": "LCIA method data set", "refObjectId": "2299222a-bbd8-474f-9d4f-4dd1f18aea7c", "version": "01.00.004", "uri": "../lciamethods/2299222a-bbd8-474f-9d4f-4dd1f18aea7c.xml"}, "meanAmount": 0.0, "other": {"anies": [{"value": "6.092530214508005E-9", "module": "A1-A3"}, {"value": "3.74803539524146E-10", "module": "A4"}, {"value": "0.0", "module": "A5"}, {"value": "0.0", "module": "B1"}, {"value": "0.0", "module": "B2"}, {"value": "0.0", "module": "B3"}, {"value": "0.0", "module": "B4"}, {"value": "0.0", "module": "B5"}, {"value": "0.0", "module": "B6"}, {"value": "0.0", "module": "B7"}, {"value": "0.0", "module": "C1", "scenario": "Thermische Verwertung"}, {"value": "1.4037585749968E-10", "module": "C2", "scenario": "Thermische Verwertung"}, {"value": "1.12611215222199E-9", "module": "C3", "scenario": "Thermische Verwertung"}, {"value": "0.0", "module": "C4", "scenario": "Thermische Verwertung"}, {"value": "-6.3972033924473E-9", "module": "D", "scenario": "Thermische Verwertung"}, {"name": "referenceToUnitGroupDataSet", "value": {"shortDescription": [{"value": "CTUh", "lang": "en"}], "type": "unit group data set", "refObjectId": "d4c9523e-2d7e-49fd-8469-998f547d3a70", "version": "00.00.003", "uri": "../unitgroups/d4c9523e-2d7e-49fd-8469-998f547d3a70.xml"}}]}}, {"referenceToLCIAMethodDataSet": {"shortDescription": [{"value": "Potential Comparative Toxic Unit for humans - non-cancer effects (HTP-nc)", "lang": "en"}, {"value": "Potenzielle Toxizitätsvergleichseinheit für den Menschen - nicht kanzerogene Wirkung (HTP-nc)", "lang": "de"}], "type": "LCIA method data set", "refObjectId": "7cfdcfcf-b222-4b26-888a-a55f9fbf7ac8", "version": "01.00.003", "uri": "../lciamethods/7cfdcfcf-b222-4b26-888a-a55f9fbf7ac8.xml"}, "meanAmount": 0.0, "other": {"anies": [{"value": "1.551191424860287E-7", "module": "A1-A3"}, {"value": "1.578901600497E-8", "module": "A4"}, {"value": "0.0", "module": "A5"}, {"value": "0.0", "module": "B1"}, {"value": "0.0", "module": "B2"}, {"value": "0.0", "module": "B3"}, {"value": "0.0", "module": "B4"}, {"value": "0.0", "module": "B5"}, {"value": "0.0", "module": "B6"}, {"value": "0.0", "module": "B7"}, {"value": "0.0", "module": "C1", "scenario": "Thermische Verwertung"}, {"value": "5.91348914043818E-9", "module": "C2", "scenario": "Thermische Verwertung"}, {"value": "5.96164137876075E-8", "module": "C3", "scenario": "Thermische Verwertung"}, {"value": "0.0", "module": "C4", "scenario": "Thermische Verwertung"}, {"value": "-1.49417399403801E-7", "module": "D", "scenario": "Thermische Verwertung"}, {"name": "referenceToUnitGroupDataSet", "value": {"shortDescription": [{"value": "CTUh", "lang": "en"}], "type": "unit group data set", "refObjectId": "d4c9523e-2d7e-49fd-8469-998f547d3a70", "version": "00.00.003", "uri": "../unitgroups/d4c9523e-2d7e-49fd-8469-998f547d3a70.xml"}}]}}, {"referenceToLCIAMethodDataSet": {"shortDescription": [{"value": "Potential Soil quality index (SQP)", "lang": "en"}, {"value": "Potenzieller Bodenqualitätsindex (SQP)", "lang": "de"}], "type": "LCIA method data set", "refObjectId": "b2ad6890-c78d-11e6-9d9d-cec0c932ce01", "version": "01.00.011", "uri": "../lciamethods/b2ad6890-c78d-11e6-9d9d-cec0c932ce01.xml"}, "meanAmount": 0.0, "other": {"anies": [{"value": "3765.9361240091275", "module": "A1-A3"}, {"value": "16.1148848904913", "module": "A4"}, {"value": "0.0", "module": "A5"}, {"value": "0.0", "module": "B1"}, {"value": "0.0", "module": "B2"}, {"value": "0.0", "module": "B3"}, {"value": "0.0", "module": "B4"}, {"value": "0.0", "module": "B5"}, {"value": "0.0", "module": "B6"}, {"value": "0.0", "module": "B7"}, {"value": "0.0", "module": "C1", "scenario": "Thermische Verwertung"}, {"value": "6.03553741216902", "module": "C2", "scenario": "Thermische Verwertung"}, {"value": "8.29618645948686", "module": "C3", "scenario": "Thermische Verwertung"}, {"value": "0.0", "module": "C4", "scenario": "Thermische Verwertung"}, {"value": "-109.880512537339", "module": "D", "scenario": "Thermische Verwertung"}, {"name": "referenceToUnitGroupDataSet", "value": {"shortDescription": [{"value": "dimensionless", "lang": "en"}], "type": "unit group data set", "refObjectId": "f130951c-e67f-4f7f-8dd4-665de3974e18", "version": "00.00.004", "uri": "../unitgroups/f130951c-e67f-4f7f-8dd4-665de3974e18.xml"}}]}}]}, "otherAttributes": {"{http://www.indata.network/EPD/2019}epd-version": "1.2", "{http://www.okworx.com/ILCD/Extensions/2018/Profile}profile": "EN_15804"}, "version": "1.1"}