{"processInformation": {"dataSetInformation": {"UUID": "c38da3ef-e75e-4d27-8794-58be29cd37ca", "name": {"baseName": [{"value": "Verbund-Sicherheitsglas EUROLAMEX", "lang": "de"}, {"value": "Laminated safety glass EUROLAMEX", "lang": "en"}], "functionalUnitFlowProperties": [{"lang": "de"}]}, "classificationInformation": {"classification": [{"class": [{"value": "Komponenten von Fenstern und Vorhangfassaden", "level": 0, "classId": "7"}, {"value": "Fenster", "level": 1, "classId": "7.8"}, {"value": "Sonstige Fenster", "level": 2, "classId": "7.8.05"}], "name": "OEKOBAU.DAT"}, {"class": [{"value": "02 Bauprodukte", "level": 0}, {"value": "Flachglas, Profilglas und Glassteinerzeugnisse", "level": 1}, {"value": "Flachglas im Bauwesen", "level": 2}], "name": "IBUCategories"}]}, "generalComment": [{"value": "Verbund-Sicherheitsglas (VSG) besteht aus mindestens zwei bereinander liegenden Glasscheiben aus Floatglas und einer oder mehreren Lagen einer reifesten und zhelastische Folie zwischen den Glasscheiben, welche in der Regel aus Polyvinylbutyral (PVB) besteht.\n\nVerbund-Sicherheitsglas bindet im Fall eines Glasbruchs Splitter und bewirkt damit eine erhebliche Reduzierung der Verletzungsgefahr.\nDarber hinaus bietet VSG im Fall des Glasbruchs eine erheblich verbesserte Resttragfhigkeit gegenber Floatglas.\nDiese EPD gilt fr folgende Produkte:\n\nProduktname Aufbau VSG\n\nEUROLAMEX 6.1 33.1 (als reprsentatives Produkt deklariert)\n\nEUROLAMEX 6.2 33.2\n\nEUROLAMEX 8.1 44.1\n\nEUROLAMEX 8.2 44.2\n\nEUROLAMEX 8.4 44,4\n\nEUROLAMEX 10.1 55.1\n\nEUROLAMEX 10.2 55.2\n\nEUROLAMEX 12.1 66.1\n\nEUROLAMEX 12.2 66.2\n\nEUROLAMEX 16.1 88.1\n\nEUROLAMEX 16.2 88.2", "lang": "de"}, {"value": "Laminated safety glass (LSG) consists of at least two superimposed panes of float glass and one or more layers of a tear-resistant and viscoplastic film between the panes, which is usually made of polyvinyl butyral (PVB).\n\nLaminated safety glass binds splinters in the event of glass breakage and thus significantly reduces the risk of injury.\nIn addition, laminated safety glass offers a significantly improved residual load-bearing capacity compared to float glass in the event of glass breakage.\n\nThis EPD applies to the following products:\n\nProduct name and build-up of the LSG\n\nEUROLAMEX 6.1 33.1 (declared as representative product)\n\nEUROLAMEX 6.2 33.2\n\nEUROLAMEX 8.1 44.1\n\nEUROLAMEX 8.2 44.2\n\nEUROLAMEX 8.4 44,4\n\nEUROLAMEX 10.1 55.1\n\nEUROLAMEX 10.2 55.2\n\nEUROLAMEX 12.1 66.1\n\nEUROLAMEX 12.2 66.2\n\nEUROLAMEX 16.1 88.1\n\nEUROLAMEX 16.2 88.2", "lang": "en"}], "other": {"anies": [{"scenario": [{"description": [{"value": "Recycling", "lang": "de"}, {"value": "Recycling", "lang": "en"}], "name": "S1", "default": true}, {"description": [{"value": "Deponierung", "lang": "de"}, {"value": "Landfilling", "lang": "en"}], "name": "S2"}]}]}}, "quantitativeReference": {"referenceToReferenceFlow": [0]}, "time": {"referenceYear": 2024, "dataSetValidUntil": 2029, "other": {"anies": [{"name": "publicationDateOfEPD", "value": 1707091200000}]}}, "geography": {"locationOfOperationSupplyOrProduction": {"location": "RER"}}, "technology": {"technologyDescriptionAndIncludedProcesses": [{"value": "Bei der Herstellung von Verbund-Sicherheitsglas werden Floatglasscheiben mittels einer PVB-Folie in einem Autoklaven unter Einwirkung von Wärme und Druck verklebt, wobei in der Glas- bzw. Foliendicke, der Glasart sowie in der Anzahl miteinander verklebter Scheiben Variationsmöglichkeiten bestehen. Im Baubereich werden meist VSG aus 2 Scheiben (und einer PVB-Folie) verwendet. Alle Standorte, an denen Floatglas und VSG hergestellt werden, sind nach EN ISO 9001 zertifiziert. \nDeklarierte Einheit: \nEs wird Verbund-Sicherheitsglas VSG EUROLAMEX 6.01 (2 Scheiben Float 3 mm, 1 Folie PVB 0,38 mm) als im Bauwesen meistverkauftes und somit reprsentatives Produkt deklariert.", "lang": "de"}, {"value": "In the production of laminated safety glass, float glass panes are bonded together using a PVB film in an autoclave under the influence of heat and pressure, with variations possible in the thickness of the glass or film, the type of glass and the number of panes bonded together. In the construction sector, laminated safety glass consisting of 2 panes (and a PVB film) is usually used. All sites where float glass and laminated safety glass are manufactured are certified to ISO 9001. \nDeclared unit: \nLaminated safety glass VSG EUROLAMEX 6.01 (2 panes of float glass 3 mm, 1 PVB film of 0.38 mm) is declared as the best-selling and therefore representative product in the construction industry.", "lang": "en"}], "technologicalApplicability": [{"value": "Verbund-Sicherheitsglas ist Ausgangsstoff fr die Herstellung einer Vielzahl von Produkten nicht nur im Bauwesen. Darunter fllt deren Verwendung als Fenster oder Fassadenelemente in der Gebudehlle oder beim Ausbau von baulichen Anlagen und Bauwerken.", "lang": "de"}, {"value": "Laminated safety glass is the starting material for the manufacture of a wide range of products, not only in the construction industry. These include their use as windows or faade elements in the building envelope or in the expansion of buildings and structures.", "lang": "en"}]}}, "modellingAndValidation": {"LCIMethodAndAllocation": {"typeOfDataSet": "EPD", "referenceToLCAMethodDetails": [{"shortDescription": [{"value": "Flachglas im Bauwesen.pdf", "lang": "de"}], "type": "source data set", "refObjectId": "51ec55ee-89fa-4ffb-8f00-767d2f4508ae"}], "other": {"anies": [{"name": "subType", "value": "average dataset"}]}}, "dataSourcesTreatmentAndRepresentativeness": {"referenceToDataSource": [{"shortDescription": [{"value": "ecoinvent database (all versions)", "lang": "de"}], "type": "source data set", "refObjectId": "b497a91f-e14b-4b69-8f28-f50eb1576766"}, {"shortDescription": [{"value": "ecoinvent 3.9.1 database", "lang": "de"}], "type": "source data set", "refObjectId": "e2034c8f-9d74-46f2-8fce-1f0c5c5cebeb"}], "useAdviceForDataSet": [{"value": "Gültigkeitsbereich: \nDie EPD deckt 100 % der Herstellung von Verbund-Sicherheitsglas der Glas Trsch Holding AG in den Werken Osterweddingen (D), Haldensleben (D) und Ujazd (PL) ab. \nSystemgrenze: \nTyp der EPD: \"von der Wiege bis zum Werkstor mit den Modulen C1–C4 und Modul D (A1–A3, C und D)\".\n\nBei der Herstellung von 2-Scheiben-Verbund-Sicherheitsglas (Module A1-A3) werden 2 Scheiben Flachglas von je 3 mm Dicke mit einer PVB-Folie verbunden. VSG wird in der Regel auf vielfach wiederverwendeten Metallstaffelein verladen; entsprechend fallen – falls berhaupt – nur geringe Mengen an Verpackungsmaterial an, das entsorgt werden muss.\nIm Zusammenhang mit der Modellierung der Herstellung von Flachglas wurden folgende Systemgrenzen im Sinne des \"Endes der Abfalleigenschaften\" angenommen:\n\nScherben werden gem VERORDNUNG (EU) Nr. 1179/2012 vom 10 Dezember 2012 als \"Produkt\" betrachtet - Glasbruch hat den Status \"Abfallende\" erreicht, wenn er als sortierter Scherben zur Verfgung steht. Externes Scherbenmaterial gelangt als sortiertes Scherbenmaterial in das Produktsystem und ist somit ein \"Sekundrmaterial\" gem EN 15804.\n\nEs wird kein Sekundrbrennstoff als Input fr die Modellierung verwendet.\n\nAufgrund der vernachlssigbaren Menge wird der Gehalt an biogenem Kohlenstoff in der Verpackung bei der Quantifizierung des Indikators \"GWP\" nicht explizit bercksichtigt (nach den Cut-off-Kriterien).\n\nDie Module A1–A3 der Produktionsstufe umfassen die Herstellung der Produkte, einschlielich der Rohstoffgewinnung und -verarbeitung, die Energieerzeugung, die Herstellung von Nebenprodukten und Verpackungsmaterialien, den Transport sowie alle Abfallbehandlungsprozesse.\n\nModul A4 wird nicht deklariert, da die bilanzierten Glser erst zu Verarbeitern und dann weiter auf die Baustelle transportiert werden; entsprechend mssen die Transporte in EPDs zu den Produkten deklariert werden, in denen Verbund-Sicherheitsglas verwendet wird.\n\nFr die eigentliche Installation werden keine Inputs und Outputs verrechnet, um Doppelzhlungen beim Verwender von Verbund-Sicherheitsglas zu vermeiden. Verbund-Sicherheitsglas wird in der Regel auf vielfach wiederverwendete Metallgestelle verladen; entsprechend fallen – falls berhaupt – nur geringe Mengen an Verpackungsmaterial an, das entsorgt werden muss; Modul A5 wird deshalb nicht deklariert.\n\nDer Unterhalt (Modul B2) des Verbund-Sicherheitsglases, namentlich dessen Reinigung, wird nicht deklariert, da er stark vom Einsatzgebiet des Verbund-Sicherheitsglases abhngt. Diese Aufwendungen mssen bei der Deklaration des Produktes bercksichtigt werden, in das das Verbund-Sicherheitsglas verbaut wird.\n\nIm End-of-Life werden 2 Szenarien deklariert:\n\nSzenario 1, Recycling: die Verwertung des rckgebauten Glases als Kiesersatz;\nSzenario 2, Entsorgung: Deponierung in einer Inertstoffdeponie.Da der Rckbau auf Stufe Endprodukt geschieht, wird Modul C1 nicht deklariert.\n\nModul C2_1 umfasst den Transport des Verbund-Sicherheitsglases (verbaut in einem Produkt) ber 50 km zu einer Sortieranlage fr Baustoffe.\n\nModul C2_2 umfasst den Transport des Verbund-Sicherheitsglases (verbaut in einem Produkt) ber 50 km auf eine Inertstoffdeponie.\n\nModul C3_1 beschreibt fr Szenario 1 die Aufbereitung des Verbund-Sicherheitsglases zu Kiesersatz.\n\nModul C4_2 beschreibt fr Szenario 2 die Deponierung des Verbund-Sicherheitsglases.\n\nModul D_1 beschreibt fr Szenario 1 die Vermeidung des Abbaus an primrem Kies, wobei eine Nettoflussberechnung im Bezug auf den Input und Output von Glasscherben vorgenommen wird.\n\nAus der Deponierung des Verbund-Sicherheitsglases ergeben sich keine Gutschriften.\n\nAuf die Deklaration von Vorteilen aus der Verwertung minimaler Abfallmengen aus der Produktion bzw. minimalen Verpackungsmengen aus Transportverpackungen wird in beiden D-Modulen verzichtet.\n\nEs werden die entsprechenden Residualmixe aus der Datenbank ecoinvent v3.9.1 verwendet, wobei das Werk Osterweddingen zertifizierten Strom aus erneuerbaren Quellen einkauft.", "lang": "de"}, {"value": "Scope: \nThe EPD covers 100% of the production of laminated safety glass by Glas Trsch Holding AG at the plants in Osterweddingen (D), Haldensleben (D) and Ujazd (PL). \nSystem boundary: \nType of EPD: \"from the cradle to the factory gate with modules C1-C4 and module D (A1-A3, C and D)\".\n\nIn the manufacture of 2-pane laminated safety glass (modules A1-A3), 2 panes of flat glass, each 3 mm thick, are bonded with a PVB film. LSG is usually loaded onto metal racks that are often reused; accordingly, only small quantities of packaging material are produced - if any at all - that have to be disposed of.\nIn connection with the modeling of the production of flat glass, the following system limits were assumed in terms of the \"end ofwaste\" status:\nCullet is considered a \"product\" according to REGULATION (EU) No. 1179/2012 of December 10, 2012. Broken glass has reached \"end of waste\" status when it is available as sorted cullet.\nExternal cullet enters the product system as sorted cullet and is therefore a \"secondary material\" according to EN 15804.\nNo secondary fuel is used as input for the modeling.\n\nDue to the negligible quantity, the content of biogenic carbon in the packaging is not explicitly taken into account when quantifying the \"GWP\" indicator (according to the cut-off criteria).\n\nModules A1-A3 of the production stage comprise the manufacture of the products, including raw material extraction and processing, energy generation, the manufacture of by-products and packaging materials, and all waste treatment processes.\n\nModule A4 is not declared, as declared glass is first transported to processors and then on to the construction site; accordingly, the transports must be declared in EPDs for the products in which laminated safety glass is used.\n\nNo inputs and outputs are attributed to the actual installation in order to avoid double counting by the user of laminated safety glass. Laminated safety glass is generally loaded onto metal racks that are often reused; accordingly, only small quantities of packaging material - if any - are produced that need to be disposed of; module A5 is therefore not declared.\n\nThe maintenance (module B2) of the laminated safety glass, namely its cleaning, is not declared, as it depends heavily on the area of application of the laminated safety glass. These inputs and outputs must be taken into account in the declaration of the product in which the laminated safety glass is installed.\n\nTwo scenarios are declared in the end-of-life:\nScenario 1, recycling: the utilization of the deconstructed glass as a gravel substitute;\nScenario 2, disposal: landfilling in an inert material landfill.As dismantling takes place at the end of life of the final product, module C1 is not declared.\n\nModule C2_1 comprises the transportation of the laminated safety glass (installed in a product) over 50 km to a sorting plant for building materials.\n\nModule C2_2 comprises the transportation of the laminated safety glass (installed in a product) over 50 km to an inert material landfill.\n\nModule C3_1 describes the processing of the laminated safety glass into gravel substitute for scenario 1.\n\nModule C4_2 describes the landfilling of the laminated safety glass for scenario 2.\n\nModule D_1 describes the avoidance of the extraction of primary gravel for scenario 1, whereby a net flow calculation is carried out in relation to the input and output of cullet.\n\nNo credits result from the landfilling of the laminated safety glass.\n\nThe declaration of benefits from the recycling of minimal quantities of waste from production or minimal quantities of packaging from transport packaging is neglected in both D-modules.\n\nThe corresponding residual mixes from the ecoinvent v3.9.1 database are used, whereby the Osterweddingen plant purchases certified electricity from renewable sources.", "lang": "en"}], "other": {"anies": [{"name": "referenceToOriginalEPD", "value": {"shortDescription": {"value": "Verbund-Sicherheitsglas EUROLAMEX.pdf", "defaultValue": "Verbund-Sicherheitsglas EUROLAMEX.pdf", "lstrings": [{"lang": "de", "value": "Verbund-Sicherheitsglas EUROLAMEX.pdf"}]}, "type": "source data set", "uuid": {"uuid": "90573868-df04-4880-8055-b827a3e6886b"}, "refObjectId": "90573868-df04-4880-8055-b827a3e6886b", "resourceURLs": ["https://oekobaudat.de/OEKOBAU.DAT/resource/sources/90573868-df04-4880-8055-b827a3e6886b/Verbund-Sicherheitsglas_EUROLAMEX_22208.pdf?version=00.02.000"]}}]}}, "validation": {"review": [{"referenceToNameOfReviewerAndInstitution": [{"shortDescription": [{"value": "Institut Bauen und Umwelt e. V.", "lang": "de"}], "type": "contact data set", "refObjectId": "d111dbec-b024-4be5-86c5-752d6eb2cf95", "uri": "../contacts/d111dbec-b024-4be5-86c5-752d6eb2cf95.xml"}], "type": "Accredited third party review"}]}, "complianceDeclarations": {"compliance": [{"referenceToComplianceSystem": {"shortDescription": [{"value": "DIN EN 15804+A2", "lang": "de"}], "type": "source data set", "refObjectId": "c0016b33-8cf7-415c-ac6e-deba0d21440d", "uri": "../sources/c0016b33-8cf7-415c-ac6e-deba0d21440d.xml"}}, {"referenceToComplianceSystem": {"shortDescription": [{"value": "ISO 14025", "lang": "de"}], "type": "source data set", "refObjectId": "4f2eb655-6e44-4874-a95a-e28f5442cd4d", "uri": "../sources/4f2eb655-6e44-4874-a95a-e28f5442cd4d.xml"}}]}}, "administrativeInformation": {"commissionerAndGoal": {"referenceToCommissioner": [{"shortDescription": [{"value": "Glas Trösch Holding AG", "lang": "de"}], "type": "contact data set", "refObjectId": "da34f235-1d94-45df-86c0-0d78d9138749", "uri": "../contacts/da34f235-1d94-45df-86c0-0d78d9138749.xml"}]}, "dataGenerator": {"referenceToPersonOrEntityGeneratingTheDataSet": [{"shortDescription": [{"value": "Dr. Frank Werner - Umwelt & Entwicklung", "lang": "de"}], "type": "contact data set", "refObjectId": "62792478-795c-4ae2-ac9a-1012d9515424", "uri": "../contacts/62792478-795c-4ae2-ac9a-1012d9515424.xml"}]}, "dataEntryBy": {"timeStamp": 1707091200000, "referenceToDataSetFormat": [{"shortDescription": [{"value": "ILCD Format", "lang": "de"}], "type": "source data set", "refObjectId": "a97a0155-0234-4b87-b4ce-a45da52f2a40", "uri": "../sources/a97a0155-0234-4b87-b4ce-a45da52f2a40.xml"}, {"shortDescription": [{"value": "EPD-Datenformaterweiterungen v1.2", "lang": "de"}, {"value": "EPD Data Format Extensions v1.2", "lang": "en"}], "type": "source data set", "refObjectId": "a29449fd-aa2f-4de8-b5d7-4b06b43c6fde", "uri": "../sources/a29449fd-aa2f-4de8-b5d7-4b06b43c6fde.xml"}]}, "publicationAndOwnership": {"dataSetVersion": "00.04.000", "referenceToRegistrationAuthority": {"shortDescription": [{"value": "Institut Bauen und Umwelt e. V.", "lang": "de"}], "type": "contact data set", "refObjectId": "d111dbec-b024-4be5-86c5-752d6eb2cf95", "uri": "../contacts/d111dbec-b024-4be5-86c5-752d6eb2cf95.xml"}, "registrationNumber": "EPD-GLS-20230183-IBB3-DE", "referenceToOwnershipOfDataSet": {"shortDescription": [{"value": "Glas Trösch Holding AG", "lang": "de"}], "type": "contact data set", "refObjectId": "da34f235-1d94-45df-86c0-0d78d9138749", "uri": "../contacts/da34f235-1d94-45df-86c0-0d78d9138749.xml"}, "copyright": true, "licenseType": "Free of charge for all users and uses", "accessRestrictions": [{"value": "None", "lang": "en"}], "other": {"anies": [{"name": "referenceToPublisher", "value": {"shortDescription": [{"value": "Institut Bauen und Umwelt e. V.", "lang": "de"}], "type": "contact data set", "refObjectId": "d111dbec-b024-4be5-86c5-752d6eb2cf95", "uri": "../contacts/d111dbec-b024-4be5-86c5-752d6eb2cf95.xml"}}]}}}, "exchanges": {"exchange": [{"dataSetInternalID": 0, "referenceToFlowDataSet": {"shortDescription": [{"value": "Verbund-Sicherheitsglas EUROLAMEX 6.1 (Verbund-Sicherheitsglas EUROLAMEX 6.1)", "lang": "de"}], "type": "flow data set", "refObjectId": "a444009e-d221-9ba4-1c4b-fb787ea1f3c9", "uri": "../flows/a444009e-d221-9ba4-1c4b-fb787ea1f3c9.xml"}, "meanAmount": 1.0, "referencesToDataSource": {}, "referenceFlow": true, "resolvedFlowVersion": "00.04.000", "resultingflowAmount": 1.0, "flowProperties": [{"name": [{"lang": "de", "value": "Fläche"}, {"lang": "en", "value": "Area"}], "uuid": "93a60a56-a3c8-19da-a746-0800200c9a66", "referenceFlowProperty": true, "meanValue": 1.0, "referenceUnit": "qm", "unitGroupUUID": "c20a03d7-bd90-4569-bc94-66cfd364dfc8"}], "materialProperties": [{"name": "grammage", "value": "15.4", "unit": "kg/m^2", "unitDescription": "kilograms per square meter"}, {"name": "layer thickness", "value": "0.00638", "unit": "m", "unitDescription": "meters"}], "typeOfFlow": "Product flow", "classification": {"classHierarchy": "Komponenten von Fenstern und Vorhangfassaden / Fenster / Sonstige Fenster", "name": "OEKOBAU.DAT"}}, {"dataSetInternalID": 1, "referenceToFlowDataSet": {"shortDescription": [{"value": "Erneuerbare Primärenergie als Energieträger (PERE)", "lang": "de"}, {"value": "Renewable primary energy as energy carrier (PERE)", "lang": "en"}], "type": "flow data set", "refObjectId": "20f32be5-0398-4288-9b6d-accddd195317", "uri": "../flows/20f32be5-0398-4288-9b6d-accddd195317.xml"}, "exchange direction": "INPUT", "other": {"anies": [{"name": "referenceToUnitGroupDataSet", "value": {"shortDescription": [{"value": "MJ", "lang": "de"}], "type": "unit group data set", "refObjectId": "93a60a57-a3c8-11da-a746-0800200c9a66", "uri": "../unitgroups/93a60a57-a3c8-11da-a746-0800200c9a66.xml"}}, {"value": "13.2260647732183", "module": "A1-A3"}, {"module": "C1"}, {"value": "0.0168781500747102", "module": "C2", "scenario": "S1"}, {"value": "0.0168781500747102", "module": "C2", "scenario": "S2"}, {"value": "0.123392829365051", "module": "C3"}, {"value": "0.0428598010595478", "module": "C4"}, {"value": "-0.203079566562975", "module": "D", "scenario": "S1"}, {"value": "0", "module": "D", "scenario": "S2"}]}, "resolvedFlowVersion": "38.00.000", "flowProperties": [], "typeOfFlow": "Other flow", "classification": {"classHierarchy": "Quantities", "name": "GaBiCategories"}}, {"dataSetInternalID": 2, "referenceToFlowDataSet": {"shortDescription": [{"value": "Erneuerbare Primärenergie zur stofflichen Nutzung (PERM)", "lang": "de"}, {"value": "Renewable primary energy resources as material utilization (PERM)", "lang": "en"}], "type": "flow data set", "refObjectId": "fb3ec0de-548d-4508-aea5-00b73bf6f702", "uri": "../flows/fb3ec0de-548d-4508-aea5-00b73bf6f702.xml"}, "exchange direction": "INPUT", "other": {"anies": [{"name": "referenceToUnitGroupDataSet", "value": {"shortDescription": [{"value": "MJ", "lang": "de"}], "type": "unit group data set", "refObjectId": "93a60a57-a3c8-11da-a746-0800200c9a66", "uri": "../unitgroups/93a60a57-a3c8-11da-a746-0800200c9a66.xml"}}, {"value": "0", "module": "A1-A3"}, {"module": "C1"}, {"value": "0", "module": "C2", "scenario": "S1"}, {"value": "0", "module": "C2", "scenario": "S2"}, {"value": "0", "module": "C3"}, {"value": "0", "module": "C4"}, {"value": "0", "module": "D", "scenario": "S1"}, {"value": "0", "module": "D", "scenario": "S2"}]}, "resolvedFlowVersion": "38.00.000", "flowProperties": [], "typeOfFlow": "Other flow", "classification": {"classHierarchy": "Quantities", "name": "GaBiCategories"}}, {"dataSetInternalID": 3, "referenceToFlowDataSet": {"shortDescription": [{"value": "Total erneuerbare Primärenergie (PERT)", "lang": "de"}, {"value": "Total use of renewable primary energy resources (PERT)", "lang": "en"}], "type": "flow data set", "refObjectId": "53f97275-fa8a-4cdd-9024-65936002acd0", "uri": "../flows/53f97275-fa8a-4cdd-9024-65936002acd0.xml"}, "exchange direction": "INPUT", "other": {"anies": [{"name": "referenceToUnitGroupDataSet", "value": {"shortDescription": [{"value": "MJ", "lang": "de"}], "type": "unit group data set", "refObjectId": "93a60a57-a3c8-11da-a746-0800200c9a66", "uri": "../unitgroups/93a60a57-a3c8-11da-a746-0800200c9a66.xml"}}, {"value": "13.2260647732183", "module": "A1-A3"}, {"module": "C1"}, {"value": "0.0168781500747102", "module": "C2", "scenario": "S1"}, {"value": "0.0168781500747102", "module": "C2", "scenario": "S2"}, {"value": "0.123392829365051", "module": "C3"}, {"value": "0.0428598010595478", "module": "C4"}, {"value": "-0.203079566562975", "module": "D", "scenario": "S1"}, {"value": "0", "module": "D", "scenario": "S2"}]}, "resolvedFlowVersion": "38.00.000", "flowProperties": [], "typeOfFlow": "Other flow", "classification": {"classHierarchy": "Quantities / Environmental quantities / EPD EN 15804 / LCI indicators", "name": "GaBiCategories"}}, {"dataSetInternalID": 4, "referenceToFlowDataSet": {"shortDescription": [{"value": "Nicht-erneuerbare Primärenergie als Energieträger (PENRE)", "lang": "de"}, {"value": "Non renewable primary energy as energy carrier (PENRE)", "lang": "en"}], "type": "flow data set", "refObjectId": "ac857178-2b45-46ec-892a-a9a4332f0372", "uri": "../flows/ac857178-2b45-46ec-892a-a9a4332f0372.xml"}, "exchange direction": "INPUT", "other": {"anies": [{"name": "referenceToUnitGroupDataSet", "value": {"shortDescription": [{"value": "MJ", "lang": "de"}], "type": "unit group data set", "refObjectId": "93a60a57-a3c8-11da-a746-0800200c9a66", "uri": "../unitgroups/93a60a57-a3c8-11da-a746-0800200c9a66.xml"}}, {"value": "204.932579792469", "module": "A1-A3"}, {"module": "C1"}, {"value": "1.17153180234847", "module": "C2", "scenario": "S1"}, {"value": "1.17153180234847", "module": "C2", "scenario": "S2"}, {"value": "1.854450941975", "module": "C3"}, {"value": "2.21504887966713", "module": "C4"}, {"value": "-0.642883349309762", "module": "D", "scenario": "S1"}, {"value": "0", "module": "D", "scenario": "S2"}]}, "resolvedFlowVersion": "38.00.000", "flowProperties": [], "typeOfFlow": "Other flow", "classification": {"classHierarchy": "Quantities", "name": "GaBiCategories"}}, {"dataSetInternalID": 5, "referenceToFlowDataSet": {"shortDescription": [{"value": "Nicht-erneuerbare Primärenergie zur stofflichen Nutzung (PENRM)", "lang": "de"}, {"value": "Non renewable primary energy as material utilization (PENRM)", "lang": "en"}], "type": "flow data set", "refObjectId": "1421caa0-679d-4bf4-b282-0eb850ccae27", "uri": "../flows/1421caa0-679d-4bf4-b282-0eb850ccae27.xml"}, "exchange direction": "INPUT", "other": {"anies": [{"name": "referenceToUnitGroupDataSet", "value": {"shortDescription": [{"value": "MJ", "lang": "de"}], "type": "unit group data set", "refObjectId": "93a60a57-a3c8-11da-a746-0800200c9a66", "uri": "../unitgroups/93a60a57-a3c8-11da-a746-0800200c9a66.xml"}}, {"value": "9.950148", "module": "A1-A3"}, {"module": "C1"}, {"value": "0", "module": "C2", "scenario": "S1"}, {"value": "0", "module": "C2", "scenario": "S2"}, {"value": "0", "module": "C3"}, {"value": "0", "module": "C4"}, {"value": "0", "module": "D", "scenario": "S1"}, {"value": "0", "module": "D", "scenario": "S2"}]}, "resolvedFlowVersion": "38.00.000", "flowProperties": [], "typeOfFlow": "Other flow", "classification": {"classHierarchy": "Quantities", "name": "GaBiCategories"}}, {"dataSetInternalID": 6, "referenceToFlowDataSet": {"shortDescription": [{"value": "Total nicht erneuerbare Primärenergie (PENRT)", "lang": "de"}, {"value": "Total use of non renewable primary energy resources (PENRT)", "lang": "en"}], "type": "flow data set", "refObjectId": "06159210-646b-4c8d-8583-da9b3b95a6c1", "uri": "../flows/06159210-646b-4c8d-8583-da9b3b95a6c1.xml"}, "exchange direction": "INPUT", "other": {"anies": [{"name": "referenceToUnitGroupDataSet", "value": {"shortDescription": [{"value": "MJ", "lang": "de"}], "type": "unit group data set", "refObjectId": "93a60a57-a3c8-11da-a746-0800200c9a66", "uri": "../unitgroups/93a60a57-a3c8-11da-a746-0800200c9a66.xml"}}, {"value": "214.882727792469", "module": "A1-A3"}, {"module": "C1"}, {"value": "1.17153180234847", "module": "C2", "scenario": "S1"}, {"value": "1.17153180234847", "module": "C2", "scenario": "S2"}, {"value": "1.854450941975", "module": "C3"}, {"value": "2.21504887966713", "module": "C4"}, {"value": "-0.642883349309762", "module": "D", "scenario": "S1"}, {"value": "0", "module": "D", "scenario": "S2"}]}, "resolvedFlowVersion": "38.00.000", "flowProperties": [], "typeOfFlow": "Other flow", "classification": {"classHierarchy": "Quantities / Environmental quantities / EPD EN 15804 / LCI indicators", "name": "GaBiCategories"}}, {"dataSetInternalID": 7, "referenceToFlowDataSet": {"shortDescription": [{"value": "Einsatz von Sekundärstoffen (SM)", "lang": "de"}, {"value": "Use of secondary material (SM)", "lang": "en"}], "type": "flow data set", "refObjectId": "c6a1f35f-2d09-4f54-8dfb-97e502e1ce92", "uri": "../flows/c6a1f35f-2d09-4f54-8dfb-97e502e1ce92.xml"}, "exchange direction": "INPUT", "other": {"anies": [{"name": "referenceToUnitGroupDataSet", "value": {"shortDescription": [{"value": "kg", "lang": "de"}], "type": "unit group data set", "refObjectId": "ad38d542-3fe9-439d-9b95-2f5f7752acaf", "uri": "../unitgroups/ad38d542-3fe9-439d-9b95-2f5f7752acaf.xml"}}, {"value": "3.17668224299065", "module": "A1-A3"}, {"module": "C1"}, {"value": "0", "module": "C2", "scenario": "S1"}, {"value": "0", "module": "C2", "scenario": "S2"}, {"value": "0", "module": "C3"}, {"value": "0", "module": "C4"}, {"value": "12.2", "module": "D", "scenario": "S1"}, {"value": "0", "module": "D", "scenario": "S2"}]}, "resolvedFlowVersion": "38.00.000", "flowProperties": [], "typeOfFlow": "Other flow", "classification": {"classHierarchy": "Quantities / Environmental quantities / EPD EN 15804 / LCI indicators", "name": "GaBiCategories"}}, {"dataSetInternalID": 8, "referenceToFlowDataSet": {"shortDescription": [{"value": "Erneuerbare Sekundärbrennstoffe (RSF)", "lang": "de"}, {"value": "Use of renewable secondary fuels (RSF)", "lang": "en"}], "type": "flow data set", "refObjectId": "64333088-a55f-4aa2-9a31-c10b07816787", "uri": "../flows/64333088-a55f-4aa2-9a31-c10b07816787.xml"}, "exchange direction": "INPUT", "other": {"anies": [{"name": "referenceToUnitGroupDataSet", "value": {"shortDescription": [{"value": "MJ", "lang": "de"}], "type": "unit group data set", "refObjectId": "93a60a57-a3c8-11da-a746-0800200c9a66", "uri": "../unitgroups/93a60a57-a3c8-11da-a746-0800200c9a66.xml"}}, {"value": "0", "module": "A1-A3"}, {"module": "C1"}, {"value": "0", "module": "C2", "scenario": "S1"}, {"value": "0", "module": "C2", "scenario": "S2"}, {"value": "0", "module": "C3"}, {"value": "0", "module": "C4"}, {"value": "0", "module": "D", "scenario": "S1"}, {"value": "0", "module": "D", "scenario": "S2"}]}, "resolvedFlowVersion": "38.00.000", "flowProperties": [], "typeOfFlow": "Other flow", "classification": {"classHierarchy": "Quantities / Environmental quantities / EPD EN 15804 / LCI indicators", "name": "GaBiCategories"}}, {"dataSetInternalID": 9, "referenceToFlowDataSet": {"shortDescription": [{"value": "Nicht erneuerbare Sekundärbrennstoffe (NRSF)", "lang": "de"}, {"value": "Use of non renewable secondary fuels (NRSF)", "lang": "en"}], "type": "flow data set", "refObjectId": "89def144-d39a-4287-b86f-efde453ddcb2", "uri": "../flows/89def144-d39a-4287-b86f-efde453ddcb2.xml"}, "exchange direction": "INPUT", "other": {"anies": [{"name": "referenceToUnitGroupDataSet", "value": {"shortDescription": [{"value": "MJ", "lang": "de"}], "type": "unit group data set", "refObjectId": "93a60a57-a3c8-11da-a746-0800200c9a66", "uri": "../unitgroups/93a60a57-a3c8-11da-a746-0800200c9a66.xml"}}, {"value": "0", "module": "A1-A3"}, {"module": "C1"}, {"value": "0", "module": "C2", "scenario": "S1"}, {"value": "0", "module": "C2", "scenario": "S2"}, {"value": "0", "module": "C3"}, {"value": "0", "module": "C4"}, {"value": "0", "module": "D", "scenario": "S1"}, {"value": "0", "module": "D", "scenario": "S2"}]}, "resolvedFlowVersion": "38.00.000", "flowProperties": [], "typeOfFlow": "Other flow", "classification": {"classHierarchy": "Quantities / Environmental quantities / EPD EN 15804 / LCI indicators", "name": "GaBiCategories"}}, {"dataSetInternalID": 10, "referenceToFlowDataSet": {"shortDescription": [{"value": "Einsatz von Süßwasserressourcen (FW)", "lang": "de"}, {"value": "Use of net fresh water (FW)", "lang": "en"}], "type": "flow data set", "refObjectId": "3cf952c8-f3a4-461d-8c96-96456ca62246", "uri": "../flows/3cf952c8-f3a4-461d-8c96-96456ca62246.xml"}, "exchange direction": "INPUT", "other": {"anies": [{"name": "referenceToUnitGroupDataSet", "value": {"shortDescription": [{"value": "m^3", "lang": "de"}], "type": "unit group data set", "refObjectId": "cd950537-0a98-4044-9ba7-9f9a68d0a504", "uri": "../unitgroups/cd950537-0a98-4044-9ba7-9f9a68d0a504.xml"}}, {"value": "0.296166670220036", "module": "A1-A3"}, {"module": "C1"}, {"value": "0.000346019733006826", "module": "C2", "scenario": "S1"}, {"value": "0.000346019733006826", "module": "C2", "scenario": "S2"}, {"value": "0.00309516060045208", "module": "C3"}, {"value": "0.000300823709095955", "module": "C4"}, {"value": "-0.00463249093433883", "module": "D", "scenario": "S1"}, {"value": "0", "module": "D", "scenario": "S2"}]}, "resolvedFlowVersion": "38.00.000", "flowProperties": [], "typeOfFlow": "Other flow", "classification": {"classHierarchy": "Quantities / Environmental quantities / EPD EN 15804 / LCI indicators", "name": "GaBiCategories"}}, {"dataSetInternalID": 11, "referenceToFlowDataSet": {"shortDescription": [{"value": "Gefährlicher Abfall zur Deponie (HWD)", "lang": "de"}, {"value": "Hazardous waste disposed (HWD)", "lang": "en"}], "type": "flow data set", "refObjectId": "430f9e0f-59b2-46a0-8e0d-55e0e84948fc", "uri": "../flows/430f9e0f-59b2-46a0-8e0d-55e0e84948fc.xml"}, "exchange direction": "OUTPUT", "other": {"anies": [{"name": "referenceToUnitGroupDataSet", "value": {"shortDescription": [{"value": "kg", "lang": "de"}], "type": "unit group data set", "refObjectId": "ad38d542-3fe9-439d-9b95-2f5f7752acaf", "uri": "../unitgroups/ad38d542-3fe9-439d-9b95-2f5f7752acaf.xml"}}, {"value": "0.00064148049628516", "module": "A1-A3"}, {"module": "C1"}, {"value": "7.27802358578504E-06", "module": "C2", "scenario": "S1"}, {"value": "7.27802358578504E-06", "module": "C2", "scenario": "S2"}, {"value": "9.18021839079752E-06", "module": "C3"}, {"value": "1.08209859361363E-05", "module": "C4"}, {"value": "-4.23775318282221E-06", "module": "D", "scenario": "S1"}, {"value": "0", "module": "D", "scenario": "S2"}]}, "resolvedFlowVersion": "38.00.000", "flowProperties": [], "typeOfFlow": "Other flow", "classification": {"classHierarchy": "Quantities / Environmental quantities / EPD EN 15804 / LCI indicators", "name": "GaBiCategories"}}, {"dataSetInternalID": 12, "referenceToFlowDataSet": {"shortDescription": [{"value": "Entsorgter nicht gefährlicher Abfall (NHWD)", "lang": "de"}, {"value": "Non hazardous waste disposed (NHWD)", "lang": "en"}], "type": "flow data set", "refObjectId": "b29ef66b-e286-4afa-949f-62f1a7b4d7fa", "uri": "../flows/b29ef66b-e286-4afa-949f-62f1a7b4d7fa.xml"}, "exchange direction": "OUTPUT", "other": {"anies": [{"name": "referenceToUnitGroupDataSet", "value": {"shortDescription": [{"value": "kg", "lang": "de"}], "type": "unit group data set", "refObjectId": "ad38d542-3fe9-439d-9b95-2f5f7752acaf", "uri": "../unitgroups/ad38d542-3fe9-439d-9b95-2f5f7752acaf.xml"}}, {"value": "1.94587616509469", "module": "A1-A3"}, {"module": "C1"}, {"value": "0.103069661023508", "module": "C2", "scenario": "S1"}, {"value": "0.103069661023508", "module": "C2", "scenario": "S2"}, {"value": "0.898232331876271", "module": "C3"}, {"value": "15.401885352277", "module": "C4"}, {"value": "-0.011958113124386", "module": "D", "scenario": "S1"}, {"value": "0", "module": "D", "scenario": "S2"}]}, "resolvedFlowVersion": "38.00.000", "flowProperties": [], "typeOfFlow": "Other flow", "classification": {"classHierarchy": "Quantities / Environmental quantities / EPD EN 15804 / LCI indicators", "name": "GaBiCategories"}}, {"dataSetInternalID": 13, "referenceToFlowDataSet": {"shortDescription": [{"value": "Entsorgter radioaktiver Abfall (RWD)", "lang": "de"}, {"value": "Radioactive waste disposed (RWD)", "lang": "en"}], "type": "flow data set", "refObjectId": "3449546e-52ad-4b39-b809-9fb77cea8ff6", "uri": "../flows/3449546e-52ad-4b39-b809-9fb77cea8ff6.xml"}, "exchange direction": "OUTPUT", "other": {"anies": [{"name": "referenceToUnitGroupDataSet", "value": {"shortDescription": [{"value": "kg", "lang": "de"}], "type": "unit group data set", "refObjectId": "ad38d542-3fe9-439d-9b95-2f5f7752acaf", "uri": "../unitgroups/ad38d542-3fe9-439d-9b95-2f5f7752acaf.xml"}}, {"value": "0.000845427056923181", "module": "A1-A3"}, {"module": "C1"}, {"value": "6.17547914801797E-07", "module": "C2", "scenario": "S1"}, {"value": "6.17547914801797E-07", "module": "C2", "scenario": "S2"}, {"value": "6.86887977290216E-06", "module": "C3"}, {"value": "8.54697831187256E-07", "module": "C4"}, {"value": "-4.38028033431069E-06", "module": "D", "scenario": "S1"}, {"value": "0", "module": "D", "scenario": "S2"}]}, "resolvedFlowVersion": "38.00.000", "flowProperties": [], "typeOfFlow": "Other flow", "classification": {"classHierarchy": "Quantities / Environmental quantities / EPD EN 15804 / LCI indicators", "name": "GaBiCategories"}}, {"dataSetInternalID": 14, "referenceToFlowDataSet": {"shortDescription": [{"value": "Komponenten für die Wiederverwendung (CRU)", "lang": "de"}, {"value": "Components for re-use (CRU)", "lang": "en"}], "type": "flow data set", "refObjectId": "a2b32f97-3fc7-4af2-b209-525bc6426f33", "uri": "../flows/a2b32f97-3fc7-4af2-b209-525bc6426f33.xml"}, "exchange direction": "OUTPUT", "other": {"anies": [{"name": "referenceToUnitGroupDataSet", "value": {"shortDescription": [{"value": "kg", "lang": "de"}], "type": "unit group data set", "refObjectId": "ad38d542-3fe9-439d-9b95-2f5f7752acaf", "uri": "../unitgroups/ad38d542-3fe9-439d-9b95-2f5f7752acaf.xml"}}, {"value": "0", "module": "A1-A3"}, {"module": "C1"}, {"value": "0", "module": "C2", "scenario": "S1"}, {"value": "0", "module": "C2", "scenario": "S2"}, {"value": "0", "module": "C3"}, {"value": "0", "module": "C4"}, {"value": "0", "module": "D", "scenario": "S1"}, {"value": "0", "module": "D", "scenario": "S2"}]}, "resolvedFlowVersion": "38.00.000", "flowProperties": [], "typeOfFlow": "Other flow", "classification": {"classHierarchy": "Quantities / Environmental quantities / EPD EN 15804 / LCI indicators", "name": "GaBiCategories"}}, {"dataSetInternalID": 15, "referenceToFlowDataSet": {"shortDescription": [{"value": "Stoffe zum Recycling (MFR)", "lang": "de"}, {"value": "Materials for recycling (MFR)", "lang": "en"}], "type": "flow data set", "refObjectId": "d7fe48a5-4103-49c8-9aae-b0b5dfdbd6ae", "uri": "../flows/d7fe48a5-4103-49c8-9aae-b0b5dfdbd6ae.xml"}, "exchange direction": "OUTPUT", "other": {"anies": [{"name": "referenceToUnitGroupDataSet", "value": {"shortDescription": [{"value": "kg", "lang": "de"}], "type": "unit group data set", "refObjectId": "ad38d542-3fe9-439d-9b95-2f5f7752acaf", "uri": "../unitgroups/ad38d542-3fe9-439d-9b95-2f5f7752acaf.xml"}}, {"value": "0", "module": "A1-A3"}, {"module": "C1"}, {"value": "0", "module": "C2", "scenario": "S1"}, {"value": "0", "module": "C2", "scenario": "S2"}, {"value": "15.4", "module": "C3"}, {"value": "0", "module": "C4"}, {"value": "0", "module": "D", "scenario": "S1"}, {"value": "0", "module": "D", "scenario": "S2"}]}, "resolvedFlowVersion": "38.00.000", "flowProperties": [], "typeOfFlow": "Other flow", "classification": {"classHierarchy": "Quantities / Environmental quantities / EPD EN 15804 / LCI indicators", "name": "GaBiCategories"}}, {"dataSetInternalID": 16, "referenceToFlowDataSet": {"shortDescription": [{"value": "Stoffe für die Energierückgewinnung (MER)", "lang": "de"}, {"value": "Materials for energy recovery (MER)", "lang": "en"}], "type": "flow data set", "refObjectId": "59a9181c-3aaf-46ee-8b13-2b3723b6e447", "uri": "../flows/59a9181c-3aaf-46ee-8b13-2b3723b6e447.xml"}, "exchange direction": "OUTPUT", "other": {"anies": [{"name": "referenceToUnitGroupDataSet", "value": {"shortDescription": [{"value": "kg", "lang": "de"}], "type": "unit group data set", "refObjectId": "ad38d542-3fe9-439d-9b95-2f5f7752acaf", "uri": "../unitgroups/ad38d542-3fe9-439d-9b95-2f5f7752acaf.xml"}}, {"value": "0", "module": "A1-A3"}, {"module": "C1"}, {"value": "0", "module": "C2", "scenario": "S1"}, {"value": "0", "module": "C2", "scenario": "S2"}, {"value": "0", "module": "C3"}, {"value": "0", "module": "C4"}, {"value": "0", "module": "D", "scenario": "S1"}, {"value": "0", "module": "D", "scenario": "S2"}]}, "resolvedFlowVersion": "38.00.000", "flowProperties": [], "typeOfFlow": "Other flow", "classification": {"classHierarchy": "Quantities / Environmental quantities / EPD EN 15804 / LCI indicators", "name": "GaBiCategories"}}, {"dataSetInternalID": 17, "referenceToFlowDataSet": {"shortDescription": [{"value": "Exportierte elektrische Energie (EEE)", "lang": "de"}, {"value": "Exported electrical energy (EEE)", "lang": "en"}], "type": "flow data set", "refObjectId": "4da0c987-2b76-40d6-9e9e-82a017aaaf29", "uri": "../flows/4da0c987-2b76-40d6-9e9e-82a017aaaf29.xml"}, "exchange direction": "OUTPUT", "other": {"anies": [{"name": "referenceToUnitGroupDataSet", "value": {"shortDescription": [{"value": "MJ", "lang": "de"}], "type": "unit group data set", "refObjectId": "93a60a57-a3c8-11da-a746-0800200c9a66", "uri": "../unitgroups/93a60a57-a3c8-11da-a746-0800200c9a66.xml"}}, {"value": "0", "module": "A1-A3"}, {"module": "C1"}, {"value": "0", "module": "C2", "scenario": "S1"}, {"value": "0", "module": "C2", "scenario": "S2"}, {"value": "0", "module": "C3"}, {"value": "0", "module": "C4"}, {"value": "0", "module": "D", "scenario": "S1"}, {"value": "0", "module": "D", "scenario": "S2"}]}, "resolvedFlowVersion": "38.00.000", "flowProperties": [], "typeOfFlow": "Other flow", "classification": {"classHierarchy": "Quantities / Environmental quantities / EPD EN 15804 / LCI indicators", "name": "GaBiCategories"}}, {"dataSetInternalID": 18, "referenceToFlowDataSet": {"shortDescription": [{"value": "Exportierte thermische Energie (EET)", "lang": "de"}, {"value": "Exported thermal energy (EET)", "lang": "en"}], "type": "flow data set", "refObjectId": "98daf38a-7a79-46d3-9a37-2b7bd0955810", "uri": "../flows/98daf38a-7a79-46d3-9a37-2b7bd0955810.xml"}, "exchange direction": "OUTPUT", "other": {"anies": [{"name": "referenceToUnitGroupDataSet", "value": {"shortDescription": [{"value": "MJ", "lang": "de"}], "type": "unit group data set", "refObjectId": "93a60a57-a3c8-11da-a746-0800200c9a66", "uri": "../unitgroups/93a60a57-a3c8-11da-a746-0800200c9a66.xml"}}, {"value": "0", "module": "A1-A3"}, {"module": "C1"}, {"value": "0", "module": "C2", "scenario": "S1"}, {"value": "0", "module": "C2", "scenario": "S2"}, {"value": "0", "module": "C3"}, {"value": "0", "module": "C4"}, {"value": "0", "module": "D", "scenario": "S1"}, {"value": "0", "module": "D", "scenario": "S2"}]}, "resolvedFlowVersion": "38.00.000", "flowProperties": [], "typeOfFlow": "Other flow", "classification": {"classHierarchy": "Quantities / Environmental quantities / EPD EN 15804 / LCI indicators", "name": "GaBiCategories"}}]}, "LCIAResults": {"LCIAResult": [{"referenceToLCIAMethodDataSet": {"shortDescription": [{"value": "Globales Erwärmungspotenzial total (GWP-total)", "lang": "de"}, {"value": "Global Warming Potential total (GWP-total)", "lang": "en"}], "type": "LCIA method data set", "refObjectId": "6a37f984-a4b3-458a-a20a-64418c145fa2", "uri": "../lciamethods/6a37f984-a4b3-458a-a20a-64418c145fa2.xml"}, "other": {"anies": [{"name": "referenceToUnitGroupDataSet", "value": {"shortDescription": [{"value": "kg CO_(2)-Äq.", "lang": "de"}], "type": "unit group data set", "refObjectId": "1ebf3012-d0db-4de2-aefd-ef30cedb0be1", "uri": "../unitgroups/1ebf3012-d0db-4de2-aefd-ef30cedb0be1.xml"}}, {"value": "16.7484745151141", "module": "A1-A3"}, {"module": "C1"}, {"value": "0.0793670031722201", "module": "C2", "scenario": "S1"}, {"value": "0.0793670031722201", "module": "C2", "scenario": "S2"}, {"value": "0.333347374548576", "module": "C3"}, {"value": "0.092733198658145", "module": "C4"}, {"value": "-0.0460489200998833", "module": "D", "scenario": "S1"}, {"value": "0", "module": "D", "scenario": "S2"}]}}, {"referenceToLCIAMethodDataSet": {"shortDescription": [{"value": "Globales Erwärmungspotenzial fossil (GWP-fossil)", "lang": "de"}, {"value": "Global Warming Potential fossil fuels (GWP-fossil)", "lang": "en"}], "type": "LCIA method data set", "refObjectId": "5f635281-343e-44fb-83df-1971b155e6b6", "uri": "../lciamethods/5f635281-343e-44fb-83df-1971b155e6b6.xml"}, "other": {"anies": [{"name": "referenceToUnitGroupDataSet", "value": {"shortDescription": [{"value": "kg CO_(2)-Äq.", "lang": "de"}], "type": "unit group data set", "refObjectId": "1ebf3012-d0db-4de2-aefd-ef30cedb0be1", "uri": "../unitgroups/1ebf3012-d0db-4de2-aefd-ef30cedb0be1.xml"}}, {"value": "16.6817740532162", "module": "A1-A3"}, {"module": "C1"}, {"value": "0.079259811623188", "module": "C2", "scenario": "S1"}, {"value": "0.079259811623188", "module": "C2", "scenario": "S2"}, {"value": "0.208493007174587", "module": "C3"}, {"value": "0.0924178892672892", "module": "C4"}, {"value": "-0.0442576415689646", "module": "D", "scenario": "S1"}, {"value": "0", "module": "D", "scenario": "S2"}]}}, {"referenceToLCIAMethodDataSet": {"shortDescription": [{"value": "Globales Erwärmungspotenzial biogen (GWP-biogenic)", "lang": "de"}, {"value": "Global Warming Potential biogenic (GWP-biogenic)", "lang": "en"}], "type": "LCIA method data set", "refObjectId": "2356e1ab-0185-4db5-86e5-16de51c7485c", "uri": "../lciamethods/2356e1ab-0185-4db5-86e5-16de51c7485c.xml"}, "other": {"anies": [{"name": "referenceToUnitGroupDataSet", "value": {"shortDescription": [{"value": "kg CO_(2)-Äq.", "lang": "de"}], "type": "unit group data set", "refObjectId": "1ebf3012-d0db-4de2-aefd-ef30cedb0be1", "uri": "../unitgroups/1ebf3012-d0db-4de2-aefd-ef30cedb0be1.xml"}}, {"value": "0.0628043328255835", "module": "A1-A3"}, {"module": "C1"}, {"value": "6.92503322175593E-05", "module": "C2", "scenario": "S1"}, {"value": "6.92503322175593E-05", "module": "C2", "scenario": "S2"}, {"value": "0.124581381191316", "module": "C3"}, {"value": "0.000298023795366044", "module": "C4"}, {"value": "-0.00175933243981972", "module": "D", "scenario": "S1"}, {"value": "0", "module": "D", "scenario": "S2"}]}}, {"referenceToLCIAMethodDataSet": {"shortDescription": [{"value": "Globales Erwärmungspotenzial luluc (GWP-luluc)", "lang": "de"}, {"value": "Global Warming Potential luluc (GWP-luluc)", "lang": "en"}], "type": "LCIA method data set", "refObjectId": "4331bbdb-978a-490d-8707-eeb047f01a55", "uri": "../lciamethods/4331bbdb-978a-490d-8707-eeb047f01a55.xml"}, "other": {"anies": [{"name": "referenceToUnitGroupDataSet", "value": {"shortDescription": [{"value": "kg CO_(2)-Äq.", "lang": "de"}], "type": "unit group data set", "refObjectId": "1ebf3012-d0db-4de2-aefd-ef30cedb0be1", "uri": "../unitgroups/1ebf3012-d0db-4de2-aefd-ef30cedb0be1.xml"}}, {"value": "0.0038961290723231", "module": "A1-A3"}, {"module": "C1"}, {"value": "3.79412168145657E-05", "module": "C2", "scenario": "S1"}, {"value": "3.79412168145657E-05", "module": "C2", "scenario": "S2"}, {"value": "0.000272986182673163", "module": "C3"}, {"value": "1.72855954897702E-05", "module": "C4"}, {"value": "-3.19460910989486E-05", "module": "D", "scenario": "S1"}, {"value": "0", "module": "D", "scenario": "S2"}]}}, {"referenceToLCIAMethodDataSet": {"shortDescription": [{"value": "Abbau Potential der stratosphärischen Ozonschicht (ODP)", "lang": "de"}, {"value": "Depletion potential of the stratospheric ozone layer (ODP)", "lang": "en"}], "type": "LCIA method data set", "refObjectId": "b5c629d6-def3-11e6-bf01-fe55135034f3", "uri": "../lciamethods/b5c629d6-def3-11e6-bf01-fe55135034f3.xml"}, "other": {"anies": [{"name": "referenceToUnitGroupDataSet", "value": {"shortDescription": [{"value": "kg CFC11-Äq.", "lang": "de"}], "type": "unit group data set", "refObjectId": "d9e957c9-7309-4474-bf3a-7777df6c4e5b", "uri": "../unitgroups/d9e957c9-7309-4474-bf3a-7777df6c4e5b.xml"}}, {"value": "4.00637296166891E-07", "module": "A1-A3"}, {"module": "C1"}, {"value": "1.75113742968218E-09", "module": "C2", "scenario": "S1"}, {"value": "1.75113742968218E-09", "module": "C2", "scenario": "S2"}, {"value": "2.14870547753653E-09", "module": "C3"}, {"value": "3.02194901879784E-09", "module": "C4"}, {"value": "-7.09826935629147E-10", "module": "D", "scenario": "S1"}, {"value": "0", "module": "D", "scenario": "S2"}]}}, {"referenceToLCIAMethodDataSet": {"shortDescription": [{"value": "Versauerungspotenzial von Boden und Wasser (AP)", "lang": "de"}, {"value": "Acidification potential of land and water (AP)", "lang": "en"}], "type": "LCIA method data set", "refObjectId": "b5c611c6-def3-11e6-bf01-fe55135034f3", "uri": "../lciamethods/b5c611c6-def3-11e6-bf01-fe55135034f3.xml"}, "other": {"anies": [{"name": "referenceToUnitGroupDataSet", "value": {"shortDescription": [{"value": "mol H^(+)-Äq.", "lang": "de"}], "type": "unit group data set", "refObjectId": "42e089ac-92bf-4bf2-8ca1-5fc40d18f2ed", "uri": "../unitgroups/42e089ac-92bf-4bf2-8ca1-5fc40d18f2ed.xml"}}, {"value": "0.09072143265496", "module": "A1-A3"}, {"module": "C1"}, {"value": "0.000191005749330202", "module": "C2", "scenario": "S1"}, {"value": "0.000191005749330202", "module": "C2", "scenario": "S2"}, {"value": "0.000691734298923352", "module": "C3"}, {"value": "0.000562920433193772", "module": "C4"}, {"value": "-0.000356736173295336", "module": "D", "scenario": "S1"}, {"value": "0", "module": "D", "scenario": "S2"}]}}, {"referenceToLCIAMethodDataSet": {"shortDescription": [{"value": "Eutrophierungspotenzial Süßwasser (EP-freshwater)", "lang": "de"}, {"value": "Eutrophication potential aquatic freshwater (EP-freshwater)", "lang": "en"}], "type": "LCIA method data set", "refObjectId": "b53ec18f-7377-4ad3-86eb-cc3f4f276b2b", "uri": "../lciamethods/b53ec18f-7377-4ad3-86eb-cc3f4f276b2b.xml"}, "other": {"anies": [{"name": "referenceToUnitGroupDataSet", "value": {"shortDescription": [{"value": "kg P-Äq.", "lang": "de"}], "type": "unit group data set", "refObjectId": "0429039d-a61d-4590-ba67-aa4a20a810a1", "uri": "../unitgroups/0429039d-a61d-4590-ba67-aa4a20a810a1.xml"}}, {"value": "0.000406269829628652", "module": "A1-A3"}, {"module": "C1"}, {"value": "6.46802101405296E-07", "module": "C2", "scenario": "S1"}, {"value": "6.46802101405296E-07", "module": "C2", "scenario": "S2"}, {"value": "3.51777235515151E-06", "module": "C3"}, {"value": "4.99300244759695E-07", "module": "C4"}, {"value": "-1.08203798482182E-06", "module": "D", "scenario": "S1"}, {"value": "0", "module": "D", "scenario": "S2"}]}}, {"referenceToLCIAMethodDataSet": {"shortDescription": [{"value": "Eutrophierungspotenzial Salzwasser (EP-marine)", "lang": "de"}, {"value": "Eutrophication potential aquatic marine (EP-marine)", "lang": "en"}], "type": "LCIA method data set", "refObjectId": "b5c619fa-def3-11e6-bf01-fe55135034f3", "uri": "../lciamethods/b5c619fa-def3-11e6-bf01-fe55135034f3.xml"}, "other": {"anies": [{"name": "referenceToUnitGroupDataSet", "value": {"shortDescription": [{"value": "kg N-Äq.", "lang": "de"}], "type": "unit group data set", "refObjectId": "d05bb823-ecdf-4686-8c40-bf1d9257859f", "uri": "../unitgroups/d05bb823-ecdf-4686-8c40-bf1d9257859f.xml"}}, {"value": "0.0135675665677807", "module": "A1-A3"}, {"module": "C1"}, {"value": "5.09641240416727E-05", "module": "C2", "scenario": "S1"}, {"value": "5.09641240416727E-05", "module": "C2", "scenario": "S2"}, {"value": "0.000273670876651905", "module": "C3"}, {"value": "0.0002446973349507", "module": "C4"}, {"value": "-0.000103951044554232", "module": "D", "scenario": "S1"}, {"value": "0", "module": "D", "scenario": "S2"}]}}, {"referenceToLCIAMethodDataSet": {"shortDescription": [{"value": "Eutrophierungspotenzial Land (EP-terrestrial)", "lang": "de"}, {"value": "Eutrophication potential terrestrial (EP-terrestrial)", "lang": "en"}], "type": "LCIA method data set", "refObjectId": "b5c614d2-def3-11e6-bf01-fe55135034f3", "uri": "../lciamethods/b5c614d2-def3-11e6-bf01-fe55135034f3.xml"}, "other": {"anies": [{"name": "referenceToUnitGroupDataSet", "value": {"shortDescription": [{"value": "mol N-Äq.", "lang": "de"}], "type": "unit group data set", "refObjectId": "71b4d617-0ec9-4d3f-b65e-e438940c2401", "uri": "../unitgroups/71b4d617-0ec9-4d3f-b65e-e438940c2401.xml"}}, {"value": "0.222764549090854", "module": "A1-A3"}, {"module": "C1"}, {"value": "0.000534238241450011", "module": "C2", "scenario": "S1"}, {"value": "0.000534238241450011", "module": "C2", "scenario": "S2"}, {"value": "0.00252432771256466", "module": "C3"}, {"value": "0.00263194379409162", "module": "C4"}, {"value": "-0.00141204322522683", "module": "D", "scenario": "S1"}, {"value": "0", "module": "D", "scenario": "S2"}]}}, {"referenceToLCIAMethodDataSet": {"shortDescription": [{"value": "Bildungspotential für troposphärisches Ozon (POCP)", "lang": "de"}, {"value": "Formation potential of tropospheric ozone photochemical oxidants (POCP)", "lang": "en"}], "type": "LCIA method data set", "refObjectId": "b5c610fe-def3-11e6-bf01-fe55135034f3", "uri": "../lciamethods/b5c610fe-def3-11e6-bf01-fe55135034f3.xml"}, "other": {"anies": [{"name": "referenceToUnitGroupDataSet", "value": {"shortDescription": [{"value": "kg NMVOC-Äq.", "lang": "de"}], "type": "unit group data set", "refObjectId": "d27c25f8-fbc1-44c6-b47b-4adbae4199c6", "uri": "../unitgroups/d27c25f8-fbc1-44c6-b47b-4adbae4199c6.xml"}}, {"value": "0.0488464866362365", "module": "A1-A3"}, {"module": "C1"}, {"value": "0.000311892637160872", "module": "C2", "scenario": "S1"}, {"value": "0.000311892637160872", "module": "C2", "scenario": "S2"}, {"value": "0.000837952227099427", "module": "C3"}, {"value": "0.00104409391043485", "module": "C4"}, {"value": "-0.000359982066729843", "module": "D", "scenario": "S1"}, {"value": "0", "module": "D", "scenario": "S2"}]}}, {"referenceToLCIAMethodDataSet": {"shortDescription": [{"value": "Potenzial für den abiotischen Abbau nicht fossiler Ressourcen (ADPE)", "lang": "de"}, {"value": "Abiotic depletion potential for non fossil resources (ADPE)", "lang": "en"}], "type": "LCIA method data set", "refObjectId": "b2ad6494-c78d-11e6-9d9d-cec0c932ce01", "uri": "../lciamethods/b2ad6494-c78d-11e6-9d9d-cec0c932ce01.xml"}, "other": {"anies": [{"name": "referenceToUnitGroupDataSet", "value": {"shortDescription": [{"value": "kg Sb-Äq.", "lang": "de"}], "type": "unit group data set", "refObjectId": "54ccd2d9-a32a-4fc2-923d-f2c8c93e89d4", "uri": "../unitgroups/54ccd2d9-a32a-4fc2-923d-f2c8c93e89d4.xml"}}, {"value": "9.61604809519735E-05", "module": "A1-A3"}, {"module": "C1"}, {"value": "2.15816435090256E-07", "module": "C2", "scenario": "S1"}, {"value": "2.15816435090256E-07", "module": "C2", "scenario": "S2"}, {"value": "5.26934273885672E-07", "module": "C3"}, {"value": "9.1845390292603E-08", "module": "C4"}, {"value": "-5.97907184851736E-07", "module": "D", "scenario": "S1"}, {"value": "0", "module": "D", "scenario": "S2"}]}}, {"referenceToLCIAMethodDataSet": {"shortDescription": [{"value": "Potenzial für den abiotischen Abbau fossiler Brennstoffe (ADPF)", "lang": "de"}, {"value": "Abiotic depletion potential for fossil resources (ADPF)", "lang": "en"}], "type": "LCIA method data set", "refObjectId": "b2ad6110-c78d-11e6-9d9d-cec0c932ce01", "uri": "../lciamethods/b2ad6110-c78d-11e6-9d9d-cec0c932ce01.xml"}, "other": {"anies": [{"name": "referenceToUnitGroupDataSet", "value": {"shortDescription": [{"value": "MJ", "lang": "de"}], "type": "unit group data set", "refObjectId": "93a60a57-a3c8-11da-a746-0800200c9a66", "uri": "../unitgroups/93a60a57-a3c8-11da-a746-0800200c9a66.xml"}}, {"value": "214.598665653436", "module": "A1-A3"}, {"module": "C1"}, {"value": "1.17115377609516", "module": "C2", "scenario": "S1"}, {"value": "1.17115377609516", "module": "C2", "scenario": "S2"}, {"value": "1.84934500239926", "module": "C3"}, {"value": "2.21481867551952", "module": "C4"}, {"value": "-0.642625741789407", "module": "D", "scenario": "S1"}, {"value": "0", "module": "D", "scenario": "S2"}]}}, {"referenceToLCIAMethodDataSet": {"shortDescription": [{"value": "Wassernutzung (WDP)", "lang": "de"}, {"value": "Water use (WDP)", "lang": "en"}], "type": "LCIA method data set", "refObjectId": "b2ad66ce-c78d-11e6-9d9d-cec0c932ce01", "uri": "../lciamethods/b2ad66ce-c78d-11e6-9d9d-cec0c932ce01.xml"}, "other": {"anies": [{"name": "referenceToUnitGroupDataSet", "value": {"shortDescription": [{"value": "m^(3) Welt-Äq. entzogen", "lang": "de"}], "type": "unit group data set", "refObjectId": "6ae2df01-888e-46c8-b17d-49fa3869b476", "uri": "../unitgroups/6ae2df01-888e-46c8-b17d-49fa3869b476.xml"}}, {"value": "8.3601385451967", "module": "A1-A3"}, {"module": "C1"}, {"value": "0.00566726003825081", "module": "C2", "scenario": "S1"}, {"value": "0.00566726003825081", "module": "C2", "scenario": "S2"}, {"value": "0.0827848022421196", "module": "C3"}, {"value": "0.00806958336786676", "module": "C4"}, {"value": "-0.0108503571117288", "module": "D", "scenario": "S1"}, {"value": "0", "module": "D", "scenario": "S2"}]}}, {"referenceToLCIAMethodDataSet": {"shortDescription": [{"value": "Auftreten von Krankheiten aufgrund von Feinstaubemissionen (PM)", "lang": "de"}, {"value": "Incidence of disease due to PM emissions (PM)", "lang": "en"}], "type": "LCIA method data set", "refObjectId": "b5c602c6-def3-11e6-bf01-fe55135034f3", "uri": "../lciamethods/b5c602c6-def3-11e6-bf01-fe55135034f3.xml"}, "other": {"anies": [{"name": "referenceToUnitGroupDataSet", "value": {"shortDescription": [{"value": "Krankheitsfälle", "lang": "de"}], "type": "unit group data set", "refObjectId": "3883559b-648f-4afc-8ba2-0bd24f3affa3", "uri": "../unitgroups/3883559b-648f-4afc-8ba2-0bd24f3affa3.xml"}}, {"value": "0.000156429356492967", "module": "A1-A3"}, {"module": "C1"}, {"value": "7.61750796561843E-09", "module": "C2", "scenario": "S1"}, {"value": "7.61750796561843E-09", "module": "C2", "scenario": "S2"}, {"value": "1.39782813332979E-08", "module": "C3"}, {"value": "1.41878967906051E-08", "module": "C4"}, {"value": "-7.78654664594087E-09", "module": "D", "scenario": "S1"}, {"value": "0", "module": "D", "scenario": "S2"}]}}, {"referenceToLCIAMethodDataSet": {"shortDescription": [{"value": "Wirkung durch Exposition des Menschen mit U235 (IR)", "lang": "de"}, {"value": "Human exposure efficiency relative to U235 (IR)", "lang": "en"}], "type": "LCIA method data set", "refObjectId": "b5c632be-def3-11e6-bf01-fe55135034f3", "uri": "../lciamethods/b5c632be-def3-11e6-bf01-fe55135034f3.xml"}, "other": {"anies": [{"name": "referenceToUnitGroupDataSet", "value": {"shortDescription": [{"value": "kBq U235-Äq.", "lang": "de"}], "type": "unit group data set", "refObjectId": "456b05bf-1415-44a9-9993-02452f554c09", "uri": "../unitgroups/456b05bf-1415-44a9-9993-02452f554c09.xml"}}, {"value": "0.282953688278186", "module": "A1-A3"}, {"module": "C1"}, {"value": "0.000563334518977785", "module": "C2", "scenario": "S1"}, {"value": "0.000563334518977785", "module": "C2", "scenario": "S2"}, {"value": "0.00503811395502676", "module": "C3"}, {"value": "0.000866528680065827", "module": "C4"}, {"value": "-0.00441606161806217", "module": "D", "scenario": "S1"}, {"value": "0", "module": "D", "scenario": "S2"}]}}, {"referenceToLCIAMethodDataSet": {"shortDescription": [{"value": "Toxizitätsvergleichseinheit für Ökosysteme (ETP-fw)", "lang": "de"}, {"value": "Comparative toxic unit for ecosystems (ETP-fw)", "lang": "en"}], "type": "LCIA method data set", "refObjectId": "ee1082d1-b0f7-43ca-a1f0-21e2a4a74511", "uri": "../lciamethods/ee1082d1-b0f7-43ca-a1f0-21e2a4a74511.xml"}, "other": {"anies": [{"name": "referenceToUnitGroupDataSet", "value": {"shortDescription": [{"value": "CTUe", "lang": "de"}], "type": "unit group data set", "refObjectId": "aa959ded-f1eb-4efb-9c5c-2d60be36b3e6", "uri": "../unitgroups/aa959ded-f1eb-4efb-9c5c-2d60be36b3e6.xml"}}, {"value": "309.614763716631", "module": "A1-A3"}, {"module": "C1"}, {"value": "0.612904629538402", "module": "C2", "scenario": "S1"}, {"value": "0.612904629538402", "module": "C2", "scenario": "S2"}, {"value": "1.50673443631267", "module": "C3"}, {"value": "0.983671363932852", "module": "C4"}, {"value": "-0.350601891514443", "module": "D", "scenario": "S1"}, {"value": "0", "module": "D", "scenario": "S2"}]}}, {"referenceToLCIAMethodDataSet": {"shortDescription": [{"value": "Toxizitätsvergleichseinheit für Menschen (krebserregend) (HTP-c)", "lang": "de"}, {"value": "Comparative toxic unit for humans (carcinogenic) (HTP-c)", "lang": "en"}], "type": "LCIA method data set", "refObjectId": "2299222a-bbd8-474f-9d4f-4dd1f18aea7c", "uri": "../lciamethods/2299222a-bbd8-474f-9d4f-4dd1f18aea7c.xml"}, "other": {"anies": [{"name": "referenceToUnitGroupDataSet", "value": {"shortDescription": [{"value": "CTUh", "lang": "de"}], "type": "unit group data set", "refObjectId": "d4c9523e-2d7e-49fd-8469-998f547d3a70", "uri": "../unitgroups/d4c9523e-2d7e-49fd-8469-998f547d3a70.xml"}}, {"value": "4.3304899570831E-09", "module": "A1-A3"}, {"module": "C1"}, {"value": "3.43255949393518E-11", "module": "C2", "scenario": "S1"}, {"value": "3.43255949393518E-11", "module": "C2", "scenario": "S2"}, {"value": "2.84990028721353E-10", "module": "C3"}, {"value": "2.95786807453483E-11", "module": "C4"}, {"value": "-8.39415127427331E-11", "module": "D", "scenario": "S1"}, {"value": "0", "module": "D", "scenario": "S2"}]}}, {"referenceToLCIAMethodDataSet": {"shortDescription": [{"value": "Toxizitätsvergleichseinheit für Menschen (nicht krebserregend) (HTP-nc)", "lang": "de"}, {"value": "Comparative toxic unit for humans (noncarcinogenic) (HTP-nc)", "lang": "en"}], "type": "LCIA method data set", "refObjectId": "3af763a5-b7a1-48c9-9cee-1f223481fcef", "uri": "../lciamethods/3af763a5-b7a1-48c9-9cee-1f223481fcef.xml"}, "other": {"anies": [{"name": "referenceToUnitGroupDataSet", "value": {"shortDescription": [{"value": "CTUh", "lang": "de"}], "type": "unit group data set", "refObjectId": "d4c9523e-2d7e-49fd-8469-998f547d3a70", "uri": "../unitgroups/d4c9523e-2d7e-49fd-8469-998f547d3a70.xml"}}, {"value": "1.66883651386767E-07", "module": "A1-A3"}, {"module": "C1"}, {"value": "1.05467280721606E-09", "module": "C2", "scenario": "S1"}, {"value": "1.05467280721606E-09", "module": "C2", "scenario": "S2"}, {"value": "2.96885830146675E-09", "module": "C3"}, {"value": "7.29916197899477E-10", "module": "C4"}, {"value": "-1.03872220268758E-09", "module": "D", "scenario": "S1"}, {"value": "0", "module": "D", "scenario": "S2"}]}}, {"referenceToLCIAMethodDataSet": {"shortDescription": [{"value": "Bodenqualitätsindex (SQP)", "lang": "de"}, {"value": "Soil quality index (SQP)", "lang": "en"}], "type": "LCIA method data set", "refObjectId": "b2ad6890-c78d-11e6-9d9d-cec0c932ce01", "uri": "../lciamethods/b2ad6890-c78d-11e6-9d9d-cec0c932ce01.xml"}, "other": {"anies": [{"name": "referenceToUnitGroupDataSet", "value": {"shortDescription": [{"value": "SQP", "lang": "de"}], "type": "unit group data set", "refObjectId": "f130951c-e67f-4f7f-8dd4-665de3974e18", "uri": "../unitgroups/f130951c-e67f-4f7f-8dd4-665de3974e18.xml"}}, {"value": "45.4697554906767", "module": "A1-A3"}, {"module": "C1"}, {"value": "1.18789215038523", "module": "C2", "scenario": "S1"}, {"value": "1.18789215038523", "module": "C2", "scenario": "S2"}, {"value": "1.56679988350811", "module": "C3"}, {"value": "4.57476153191407", "module": "C4"}, {"value": "-1.26889243010555", "module": "D", "scenario": "S1"}, {"value": "0", "module": "D", "scenario": "S2"}]}}]}, "otherAttributes": {"{http://www.indata.network/EPD/2019}epd-version": "1.2"}, "version": "1.1", "locations": "../ILCDLocations.xml"}