{"processInformation": {"dataSetInformation": {"UUID": "c5d07bee-d468-4468-bd69-93f019a4123b", "name": {"baseName": [{"value": "HALFEN Iso-ElemenT HIT-HP/SP", "lang": "en"}, {"value": "HALFEN Iso-ElemenT HIT-HP/SP", "lang": "de"}], "functionalUnitFlowProperties": [{"lang": "en"}]}, "classificationInformation": {"classification": [{"class": [{"value": "Dämmstoffe", "level": 0, "classId": "2"}, {"value": "Dämmelemente", "level": 1, "classId": "2.25"}, {"value": "Isokörbe", "level": 2, "classId": "2.25.01"}], "name": "OEKOBAU.DAT"}, {"class": [{"value": "02 Building products", "level": 0}, {"value": "Thermal insulation products", "level": 1}, {"value": "Load-bearing thermal insulation elements", "level": 2}], "name": "IBUCategories"}]}, "generalComment": [{"value": "The HALFEN Iso-ElemenT HIT-HP/SP is a load bearing insulated connection element for thermal separation of reinforced concrete components such as e.g. balcony and ceiling slabs. It is used to prevent mould, to ensure increased building physical requirements and to avoid cracking due to temperature expansions. It consists of a sturdy casing box made of plastic, which is filled with mineral rock wool. In addition to the insulating effect, the mineral rock wool is used as fireproofing material so that all versions of the insulated connection element HIT-HP/SP are by default classified in the fire resistance class REI 120 according to /EN 13501-2/.\n\nDepending on the element type the load bearings such as e.g. tension bars, compression bars or studs, shear bars and Compression-Shear-Bearings (CSB) form the statically bearing components of the system. They are arranged into the casing box in such a way that a shift in all three spatial directions can be excluded, so that the system has a high assembly security. The element type and the load-bearing level depend on the required load. The load-bearing elements and their numbers vary depending on the element type and load-bearing level.\n\nThe steel components are made of stainless steel or a combination of stainless steel and rebars. The Compression-Shear-Bearings consist of a fibre-reinforced high-performance mortar and are adapted with regard to the usage area, as well as mechanical and structural properties.\n\nThe HALFEN Iso-ElemenT HIT-HP/SP is available in the following variants:\n\nJoint widths: HP = 80 mm, SP = 120 mm\nNumber and diameter of tension bars, compression bars / studs and shear bars\nNumber of compression-shear-bearings\nElement height\nElement length\nConcrete coverThe respective variant of HALFEN Iso-ElemenT HIT is integrated in the product name and so clearly defined.\nThe declared product HIT-SP MVX-0805-20-100-cc in the EPD is thus characterized by:\n\nJoint widths: SP = 120 mm\nNumber of tension bars: 8  12 mm\nNumber of compression-shear-bearings: 5\nElement height: h = 20 cm\nElement length: l = 100 cm\nConcrete cover: cc ≥ 30 mmDetailed information about HALFEN Iso-ElemenT HIT-SP MVX-0805-20-100-cc is included in the table in section 2.3.", "lang": "en"}, {"value": "Das HALFEN Iso-ElemenT HIT-HP/SP ist ein tragendes isoliertes Anschlusselement zur thermischen Trennung von Stahlbetonbauteilen wie z.B. Balkon- und Deckenplatten. Es wird eingesetzt, um Schimmel zu verhindern, erhöhte bauphysikalische Anforderungen zu gewährleisten und Rissbildung aufgrund von Temperaturausdehnungen zu vermeiden. Es besteht aus einem stabilen Verwahrkasten aus Kunststoff, der mit mineralischer Steinwolle gefüllt ist. Zusätzlich zur Dämmwirkung wird die Mineralwolle als Brandschutzmaterial eingesetzt, so dass alle Varianten des gedämmten Anschlusselements HIT-HP/SP standardmäßig in die Feuerwiderstandsklasse REI 120 nach /EN 13501-2/ eingestuft sind. Je nach Elementtyp bilden die Tragglieder wie z.B. Zugstäbe, Druckstäbe oder -lager, Querkraftstäbe und Druck-Schublager (CSB) die statisch tragenden Komponenten des Systems. Sie sind so im Verwahrkasten angeordnet, dass eine Verschiebung in alle drei Raumrichtungen ausgeschlossen werden kann, so dass das System eine hohe Montagesicherheit aufweist. Die Art der Elemente und die Höhe der Tragfähigkeit hängen von der erforderlichen Belastung ab. Die tragenden Elemente und ihre Anzahl variieren je nach Elementtyp und Belastungsgrad. Die Stahlelemente sind aus rostfreiem Stahl oder einer Kombination aus rostfreiem Stahl und Bewehrungsstäben gefertigt. Die Druck-Schub-Lager bestehen aus einem faserverstärkten Hochleistungsmörtel und sind hinsichtlich des Einsatzbereiches sowie der mechanischen und statischen Eigenschaften angepasst. Das HALFEN Iso-ElemenT HIT-HP/SP ist in folgenden Varianten erhältlich: Fugenbreiten: HP = 80 mm, SP = 120 mm, Anzahl und Durchmesser von Zugstäben, Druckstäben / -lager und Querkraftstäben Anzahl der Druck-Schublager, Elementhöhe, Elementlänge, Betondeckung. Die jeweilige Variante des HALFEN Iso-ElemenT HIT ist im Produktnamen integriert und somit eindeutig definiert. Das in der EPD deklarierte Produkt HIT-SP MVX-0805-20-100-cc ist somit gekennzeichnet durch: Fugenbreiten: SP = 120 mm, Anzahl der Zugstäbe: 8 Ø 12 mm, Anzahl der Druck-Schublager: 5, Elementhöhe: h = 20 cm, Elementlänge: l = 100 cm, Betondeckung: cc ≥ 30 mm. Detaillierte Informationen zu HALFEN Iso-ElemenT HIT-SP MVX-0805-20-100-cc finden Sie in der Tabelle in Abschnitt 2.3.", "lang": "de"}]}, "quantitativeReference": {"referenceToReferenceFlow": [0]}, "time": {"referenceYear": 2023, "dataSetValidUntil": 2028, "other": {"anies": [{"name": "publicationDateOfEPD", "value": 1693872000000}]}}, "geography": {"locationOfOperationSupplyOrProduction": {"location": "RER"}}, "technology": {"technologyDescriptionAndIncludedProcesses": [{"value": "The materials needed for the final assembly of the HALFEN Iso-ElemenT HIT-HP/SP are manufactured in-house or purchased from qualified vendors. The Halfen Iso-ElemenT HIT-HP/SP is constructed from a modular system of plastic enclosures with integrated heat-insulating fire protection material. To be protected against moisture, the heat-insulating fire protection material is enclosed in the housing box from all sides. Welded joints are made using recognised and certified welding procedures, mostly with automatic welding machines. Necessary bends, such as for the shear bars, are realised with automatic bending machines. The compression-shear bearings made of high-performance mortar are manufactured in the Leviat plant in Kalisz / Poland. A large part of the stainless steel sections of the tension and compression bars are manufactured in the Leviat plant in Artern / Germany. The components, processed casing boxes and assembled module units are produced at Leviat plant in Kalisz / Poland. The final assembling of all module units is done at Leviat plant in Artern / Germany, Leviat plant in Kalisz / Poland or directly by selected customers. \nTechnical data: \nThe detailed technical information of the individual HALFEN Iso-ElemenTs HIT-HP/SP depends on the load capacity as well as the element type and can be found in the related technical information on the website www.halfen.com. \nDeclared unit: \nThe declared unit is 1 m length of load bearing thermal insulation element HALFEN Iso-ElemenT Type HIT-SP MVX-0805-20-100-cc.\nThe calculation of the average of two production sites is based on actual production volumes.", "lang": "en"}, {"value": "Die Materialien, die für die Endmontage des HALFEN Iso-ElemenT HIT-HP/SP benötigt werden, werden entweder selbst hergestellt oder von qualifizierten Anbietern bezogen.\n\nDas Halfen Iso-ElemenT HIT-HP/SP ist aus einem modularen System von Kunststoffgehäusen mit integriertem wärmedämmendem Brandschutzmaterial aufgebaut. Um vor Feuchtigkeit geschützt zu sein, ist das wärmedämmende Brandschutzmaterial von allen Seiten in den Verwahrkasten eingeschlossen.\n\nDie Schweißnähte werden mit anerkannten und zertifizierten Schweißverfahren, meist mit Schweißautomaten, hergestellt. Notwendige Biegungen, z.B. für die Querkraftstäbe, werden mit Biegeautomaten realisiert. Die Druck-Schublager aus Hochleistungsmörtel werden im Leviat-Werk in Kalisz / Polen hergestellt. Ein großer Teil der nichtrostenden Stahlelemente der Zug- und Druckstäbe wird im Leviat-Werk in Artern / Deutschland hergestellt.\n\nDie Komponenten, die bearbeiteten Verwahrkästen und die montierten Moduleinheiten werden im Leviat-Werk in Kalisz / Polen hergestellt.\n\nDie Endmontage aller Moduleinheiten erfolgt im Leviat-Werk in Artern / Deutschland, im Leviat-Werk in Kalisz / Polen oder direkt bei ausgewählten Kunden. \nTechnische Daten: \nDie detaillierten technischen Informationen der einzelnen HALFEN Iso-ElemenTs HIT-HP/SP sind abhängig von der Tragfähigkeit sowie dem Elementtyp und können den entsprechenden technischen Informationen auf der Website www.halfen.com entnommen werden. \nDeklarierte Einheit: \nDie deklarierte Einheit ist 1 m Länge des tragenden Wärmedämmelements HALFEN Iso-ElemenT Typ HIT-SP MVX-0805-20-100-cc. Die Berechnung des Durchschnitts von zwei Produktionsstätten basiert auf den tatsächlichen Produktionsmengen.", "lang": "de"}], "technologicalApplicability": [{"value": "The HALFEN Iso-ElemenT HIT-HP/SP is used for static transfer of bending moments and/or shear forces and/or compression or tension forces. It is placed between the outer and inner reinforced concrete construction such that the heat flow is locally minimized, and the thermal bridges are reduced. The construction of the HALFEN Iso-ElemenTs, which is optimized for the respective application situation, ensures effective thermal insulation and impact sound reduction. This is shown with various characteristic values.", "lang": "en"}, {"value": "Das HALFEN Iso-ElemenT HIT-HP/SP wird zur statischen Übertragung von Biegemomenten und / oder Querkräften und / oder Druck- oder Zugkräften eingesetzt. Er wird zwischen der äußeren und inneren Stahlbetonkonstruktion platziert, so dass der Wärmefluss lokal minimiert wird und die Wärmebrücken reduziert werden. Die für die jeweilige Anwendungssituation optimierte Konstruktion der HALFEN Iso-ElemenTs sorgt für eine effektive Wärmedämmung und Trittschallminderung. Dies wird mit verschiedenen Kennwerten gezeigt.", "lang": "de"}]}}, "modellingAndValidation": {"LCIMethodAndAllocation": {"typeOfDataSet": "EPD", "referenceToLCAMethodDetails": [{"shortDescription": [{"value": "Load-bearing thermal insulation elements.pdf", "lang": "en"}], "type": "source data set", "refObjectId": "44f2615d-5fd0-44ea-b218-dd49bf158137"}], "other": {"anies": [{"name": "subType", "value": "specific dataset"}]}}, "dataSourcesTreatmentAndRepresentativeness": {"referenceToDataSource": [{"shortDescription": [{"value": "GaBi Database (all versions)", "lang": "en"}], "type": "source data set", "refObjectId": "28d74cc0-db8b-4d7e-bc44-5f6d56ce0c4a"}, {"shortDescription": [{"value": "GaBi Database Edition 2022, CUP 2022.02", "lang": "en"}], "type": "source data set", "refObjectId": "94f442cb-662e-43ea-a792-4b0a35132e93"}], "useAdviceForDataSet": [{"value": "Scope: \nThis EPD refers to the specific load-bearing thermally insulated connection element HALFEN Iso-ElemenT type HIT-SP MVX-0805-20-100-cc manufactured by Leviat.\n\nSome stainless steel components are produced at Leviat plant Artern / Germany.\nOther components and assembled module units are produced at Leviat plant Kalisz / Poland. The final assembling of all module units is done at Leviat plant Artern / Germany or at Leviat plant Kalisz / Poland.\n\nThe results of this EPD and the annex can be applied to other products of the HALFEN Iso-ElemenT family. \nSystem boundary: \nType of the EPD: cradle-to-gate - with options, modules C1-C4 and module D (A1-A3 + C + D and additional modules: A4, A5).\nProduction Stage (A1-A3): The Product stage includes:\nA1 Raw material supply and processing (mainly steel and PVC-parts),\n\nA2 Transport of raw materials to the manufacturer,\n\nA3 Production of HIT-HP/SP in the factory, (incl. energy provision, water provision, treatment of production waste, production of packaging materials)Construction stage (A4-A5): The construction process stage includes:\n\nA4 transport to the construction site 100km by truck,\n\nA5 Disposal of the packaging after installation of the HIT-HP/SPEnd-of-life stage (C1-C4): The end-of-life stage includes:\n\nC1 machine-assisted de- construction (demolition excavator - diesel-powered)\n\nC2 transport to waste processing; 50 km by truck. Transport distance can be adjusted at building level if necessary (e.g., for 100 km actual transport distance: multiply LCA values by factor 2).\n\nC3 waste processing for incineration of plastic components, recycling of metals\n\nC4 disposal of inert material (except metals)Benefits and loads beyond the System Boundary (D): Module D includes:\nMaterial recovery potentials from metal recycling and energy recovery potentials from the thermal recycling of the mixed plastic waste.", "lang": "en"}, {"value": "Gültigkeitsbereich: \nDiese EPD bezieht sich auf das spezifische tragende wärmegedämmte Anschlusselement HALFEN Iso-ElemenT vom Typ HIT-SP MVX-0805-20-100-cc, das von Leviat hergestellt wird. Einige nichtrostende Stahlkomponenten werden im Leviat-Werk Artern / Deutschland hergestellt. Andere Komponenten sowie Moduleinheiten werden im Leviat-Werk Kalisz / Polen hergestellt. Die Endmontage aller Moduleinheiten erfolgt im Leviat Werk Artern / Deutschland oder im Leviat Werk Kalisz / Polen. Die Ergebnisse dieser EPD und des Anhangs können auf andere Produkte der HALFEN Iso-ElemenT Familie angewendet werden. \nSystemgrenze: \nArt der EPD: Cradle-to-Gate - mit Optionen, Modulen C1-C4 und Modul D (A1-A3 + C + D und zusätzliche Module: A4, A5). Produktionsstufe (A1-A3): Die Produktphase umfasst: A1 Rohstoffbeschaffung und -verarbeitung (hauptsächlich Stahl- und PVC-Teile), A2 Transport der Rohstoffe zum Hersteller, A3 Produktion von HIT-HP/SP in der Fabrik, (inkl. Energieversorgung, Wasserversorgung, Behandlung von Produktionsabfällen, Herstellung von Verpackungsmaterialien) Bauphase (A4-A5): Die Bauprozessphase umfasst: A4 Transport zur Baustelle 100km mit LKW, A5 Entsorgung der Verpackung nach der Installation des HIT-HP/SP Lebensendephase (C1-C4): Die End-of-Life-Phase umfasst: C1 maschinengestützter Rückbau (Abbruchbagger - dieselbetrieben) C2 Transport zur Abfallverarbeitung; 50 km mit LKW. Die Transportdistanz kann bei Bedarf auf Gebäudeebene angepasst werden (z.B. für 100 km tatsächliche Transportdistanz: LCA-Werte mit Faktor 2 multiplizieren). C3 Abfallverarbeitung zur Verbrennung von Kunststoffkomponenten, Recycling von Metallen C4 Entsorgung von Inertmaterial (außer Metallen) Nutzen und Lasten jenseits der Systemgrenze (D): Modul D umfasst: Materialrückgewinnungspotenziale aus dem Metallrecycling und Energierückgewinnungspotenziale aus dem thermischen Recycling der gemischten Kunststoffabfälle.", "lang": "de"}], "other": {"anies": [{"name": "referenceToOriginalEPD", "value": {"shortDescription": {"value": "HALFEN Iso-ElemenT HIT-HP/SP.pdf", "defaultValue": "HALFEN Iso-ElemenT HIT-HP/SP.pdf", "lstrings": [{"lang": "en", "value": "HALFEN Iso-ElemenT HIT-HP/SP.pdf"}]}, "type": "source data set", "uuid": {"uuid": "dada4ed1-190e-4570-8d3b-6017ce435638"}, "refObjectId": "dada4ed1-190e-4570-8d3b-6017ce435638", "resourceURLs": ["https://oekobaudat.de/OEKOBAU.DAT/resource/sources/dada4ed1-190e-4570-8d3b-6017ce435638/HALFEN_Iso-ElemenT_HIT-HPSP_15956.pdf?version=00.01.000"]}}]}}, "validation": {"review": [{"referenceToNameOfReviewerAndInstitution": [{"shortDescription": [{"value": "Institut Bauen und Umwelt e. V.", "lang": "en"}], "type": "contact data set", "refObjectId": "d111dbec-b024-4be5-86c5-752d6eb2cf95", "uri": "../contacts/d111dbec-b024-4be5-86c5-752d6eb2cf95.xml"}], "type": "Accredited third party review"}]}, "complianceDeclarations": {"compliance": [{"referenceToComplianceSystem": {"shortDescription": [{"value": "DIN EN 15804+A2", "lang": "en"}], "type": "source data set", "refObjectId": "c0016b33-8cf7-415c-ac6e-deba0d21440d", "uri": "../sources/c0016b33-8cf7-415c-ac6e-deba0d21440d.xml"}}, {"referenceToComplianceSystem": {"shortDescription": [{"value": "ISO 14025", "lang": "en"}], "type": "source data set", "refObjectId": "4f2eb655-6e44-4874-a95a-e28f5442cd4d", "uri": "../sources/4f2eb655-6e44-4874-a95a-e28f5442cd4d.xml"}}]}}, "administrativeInformation": {"commissionerAndGoal": {"referenceToCommissioner": [{"shortDescription": [{"value": "Leviat GmbH", "lang": "en"}], "type": "contact data set", "refObjectId": "a6732492-15a9-4454-a40d-69bdbca38cd1", "uri": "../contacts/a6732492-15a9-4454-a40d-69bdbca38cd1.xml"}]}, "dataGenerator": {"referenceToPersonOrEntityGeneratingTheDataSet": [{"shortDescription": [{"value": "Sphera Solutions GmbH", "lang": "en"}], "type": "contact data set", "refObjectId": "623edf96-39d1-4e6f-9892-674c7228546b", "uri": "../contacts/623edf96-39d1-4e6f-9892-674c7228546b.xml"}]}, "dataEntryBy": {"timeStamp": 1693872000000, "referenceToDataSetFormat": [{"shortDescription": [{"value": "ILCD Format", "lang": "en"}], "type": "source data set", "refObjectId": "a97a0155-0234-4b87-b4ce-a45da52f2a40", "uri": "../sources/a97a0155-0234-4b87-b4ce-a45da52f2a40.xml"}, {"shortDescription": [{"value": "EPD-Datenformaterweiterungen v1.2", "lang": "de"}, {"value": "EPD Data Format Extensions v1.2", "lang": "en"}], "type": "source data set", "refObjectId": "a29449fd-aa2f-4de8-b5d7-4b06b43c6fde", "uri": "../sources/a29449fd-aa2f-4de8-b5d7-4b06b43c6fde.xml"}]}, "publicationAndOwnership": {"dataSetVersion": "00.01.000", "referenceToRegistrationAuthority": {"shortDescription": [{"value": "Institut Bauen und Umwelt e. V.", "lang": "en"}], "type": "contact data set", "refObjectId": "d111dbec-b024-4be5-86c5-752d6eb2cf95", "uri": "../contacts/d111dbec-b024-4be5-86c5-752d6eb2cf95.xml"}, "registrationNumber": "EPD-HAL-20230142-IBC1-EN", "referenceToOwnershipOfDataSet": {"shortDescription": [{"value": "Leviat GmbH", "lang": "en"}], "type": "contact data set", "refObjectId": "a6732492-15a9-4454-a40d-69bdbca38cd1", "uri": "../contacts/a6732492-15a9-4454-a40d-69bdbca38cd1.xml"}, "copyright": true, "licenseType": "Free of charge for all users and uses", "accessRestrictions": [{"value": "None", "lang": "en"}], "other": {"anies": [{"name": "referenceToPublisher", "value": {"shortDescription": [{"value": "Institut Bauen und Umwelt e. V.", "lang": "en"}], "type": "contact data set", "refObjectId": "d111dbec-b024-4be5-86c5-752d6eb2cf95", "uri": "../contacts/d111dbec-b024-4be5-86c5-752d6eb2cf95.xml"}}]}}}, "exchanges": {"exchange": [{"dataSetInternalID": 0, "referenceToFlowDataSet": {"shortDescription": [{"value": "HALFEN Iso-ElemenT HIT-HP/SP, 1m ()", "lang": "en"}], "type": "flow data set", "refObjectId": "4ba8cd64-c009-1753-f596-6fb26dc0c151", "uri": "../flows/4ba8cd64-c009-1753-f596-6fb26dc0c151.xml"}, "meanAmount": 1.0, "referencesToDataSource": {}, "referenceFlow": true, "resolvedFlowVersion": "00.01.000", "resultingflowAmount": 1.0, "flowProperties": [{"name": [{"lang": "de", "value": "Länge"}, {"lang": "en", "value": "Length"}], "uuid": "838aaa23-0117-11db-92e3-0800200c9a66", "referenceFlowProperty": true, "meanValue": 1.0, "referenceUnit": "m", "unitGroupUUID": "838aaa22-0117-11db-92e3-0800200c9a66"}], "materialProperties": [{"name": "linear density", "value": "21.42", "unit": "kg/m"}], "typeOfFlow": "Product flow", "classification": {"classHierarchy": "Dämmstoffe / Dämmelemente / Isokörbe", "name": "OEKOBAU.DAT"}}, {"dataSetInternalID": 1, "referenceToFlowDataSet": {"shortDescription": [{"value": "Renewable primary energy as energy carrier (PERE)", "lang": "en"}, {"value": "Erneuerbare Primärenergie als Energieträger (PERE)", "lang": "de"}], "type": "flow data set", "refObjectId": "20f32be5-0398-4288-9b6d-accddd195317", "uri": "../flows/20f32be5-0398-4288-9b6d-accddd195317.xml"}, "exchange direction": "INPUT", "other": {"anies": [{"name": "referenceToUnitGroupDataSet", "value": {"shortDescription": [{"value": "MJ", "lang": "en"}], "type": "unit group data set", "refObjectId": "93a60a57-a3c8-11da-a746-0800200c9a66", "uri": "../unitgroups/93a60a57-a3c8-11da-a746-0800200c9a66.xml"}}, {"value": "89.32", "module": "A1-A3"}, {"value": "0.13", "module": "A4"}, {"value": "10", "module": "A5"}, {"value": "0.0122", "module": "C1"}, {"value": "0.065", "module": "C2"}, {"value": "4.78", "module": "C3"}, {"value": "0.187", "module": "C4"}, {"value": "-15.6", "module": "D"}]}, "resolvedFlowVersion": "38.00.000", "flowProperties": [], "typeOfFlow": "Other flow", "classification": {"classHierarchy": "Quantities", "name": "GaBiCategories"}}, {"dataSetInternalID": 2, "referenceToFlowDataSet": {"shortDescription": [{"value": "Renewable primary energy resources as material utilization (PERM)", "lang": "en"}, {"value": "Erneuerbare Primärenergie zur stofflichen Nutzung (PERM)", "lang": "de"}], "type": "flow data set", "refObjectId": "fb3ec0de-548d-4508-aea5-00b73bf6f702", "uri": "../flows/fb3ec0de-548d-4508-aea5-00b73bf6f702.xml"}, "exchange direction": "INPUT", "other": {"anies": [{"name": "referenceToUnitGroupDataSet", "value": {"shortDescription": [{"value": "MJ", "lang": "en"}], "type": "unit group data set", "refObjectId": "93a60a57-a3c8-11da-a746-0800200c9a66", "uri": "../unitgroups/93a60a57-a3c8-11da-a746-0800200c9a66.xml"}}, {"value": "9.98", "module": "A1-A3"}, {"value": "0", "module": "A4"}, {"value": "-9.98", "module": "A5"}, {"value": "0", "module": "C1"}, {"value": "0", "module": "C2"}, {"value": "0", "module": "C3"}, {"value": "0", "module": "C4"}, {"value": "0", "module": "D"}]}, "resolvedFlowVersion": "38.00.000", "flowProperties": [], "typeOfFlow": "Other flow", "classification": {"classHierarchy": "Quantities", "name": "GaBiCategories"}}, {"dataSetInternalID": 3, "referenceToFlowDataSet": {"shortDescription": [{"value": "Total use of renewable primary energy resources (PERT)", "lang": "en"}, {"value": "Total erneuerbare Primärenergie (PERT)", "lang": "de"}], "type": "flow data set", "refObjectId": "53f97275-fa8a-4cdd-9024-65936002acd0", "uri": "../flows/53f97275-fa8a-4cdd-9024-65936002acd0.xml"}, "exchange direction": "INPUT", "other": {"anies": [{"name": "referenceToUnitGroupDataSet", "value": {"shortDescription": [{"value": "MJ", "lang": "en"}], "type": "unit group data set", "refObjectId": "93a60a57-a3c8-11da-a746-0800200c9a66", "uri": "../unitgroups/93a60a57-a3c8-11da-a746-0800200c9a66.xml"}}, {"value": "99.32", "module": "A1-A3"}, {"value": "0.13", "module": "A4"}, {"value": "0.0199999999999996", "module": "A5"}, {"value": "0.0122", "module": "C1"}, {"value": "0.065", "module": "C2"}, {"value": "4.78", "module": "C3"}, {"value": "0.187", "module": "C4"}, {"value": "-15.6", "module": "D"}]}, "resolvedFlowVersion": "38.00.000", "flowProperties": [], "typeOfFlow": "Other flow", "classification": {"classHierarchy": "Quantities / Environmental quantities / EPD EN 15804 / LCI indicators", "name": "GaBiCategories"}}, {"dataSetInternalID": 4, "referenceToFlowDataSet": {"shortDescription": [{"value": "Non renewable primary energy as energy carrier (PENRE)", "lang": "en"}, {"value": "Nicht-erneuerbare Primärenergie als Energieträger (PENRE)", "lang": "de"}], "type": "flow data set", "refObjectId": "ac857178-2b45-46ec-892a-a9a4332f0372", "uri": "../flows/ac857178-2b45-46ec-892a-a9a4332f0372.xml"}, "exchange direction": "INPUT", "other": {"anies": [{"name": "referenceToUnitGroupDataSet", "value": {"shortDescription": [{"value": "MJ", "lang": "en"}], "type": "unit group data set", "refObjectId": "93a60a57-a3c8-11da-a746-0800200c9a66", "uri": "../unitgroups/93a60a57-a3c8-11da-a746-0800200c9a66.xml"}}, {"value": "389", "module": "A1-A3"}, {"value": "1.88", "module": "A4"}, {"value": "0.225", "module": "A5"}, {"value": "0.176", "module": "C1"}, {"value": "0.942", "module": "C2"}, {"value": "145", "module": "C3"}, {"value": "1.25", "module": "C4"}, {"value": "-104", "module": "D"}]}, "resolvedFlowVersion": "38.00.000", "flowProperties": [], "typeOfFlow": "Other flow", "classification": {"classHierarchy": "Quantities", "name": "GaBiCategories"}}, {"dataSetInternalID": 5, "referenceToFlowDataSet": {"shortDescription": [{"value": "Non renewable primary energy as material utilization (PENRM)", "lang": "en"}, {"value": "Nicht-erneuerbare Primärenergie zur stofflichen Nutzung (PENRM)", "lang": "de"}], "type": "flow data set", "refObjectId": "1421caa0-679d-4bf4-b282-0eb850ccae27", "uri": "../flows/1421caa0-679d-4bf4-b282-0eb850ccae27.xml"}, "exchange direction": "INPUT", "other": {"anies": [{"name": "referenceToUnitGroupDataSet", "value": {"shortDescription": [{"value": "MJ", "lang": "en"}], "type": "unit group data set", "refObjectId": "93a60a57-a3c8-11da-a746-0800200c9a66", "uri": "../unitgroups/93a60a57-a3c8-11da-a746-0800200c9a66.xml"}}, {"value": "127", "module": "A1-A3"}, {"value": "0", "module": "A4"}, {"value": "0", "module": "A5"}, {"value": "0", "module": "C1"}, {"value": "0", "module": "C2"}, {"value": "-127", "module": "C3"}, {"value": "0", "module": "C4"}, {"value": "0", "module": "D"}]}, "resolvedFlowVersion": "38.00.000", "flowProperties": [], "typeOfFlow": "Other flow", "classification": {"classHierarchy": "Quantities", "name": "GaBiCategories"}}, {"dataSetInternalID": 6, "referenceToFlowDataSet": {"shortDescription": [{"value": "Total use of non renewable primary energy resources (PENRT)", "lang": "en"}, {"value": "Total nicht erneuerbare Primärenergie (PENRT)", "lang": "de"}], "type": "flow data set", "refObjectId": "06159210-646b-4c8d-8583-da9b3b95a6c1", "uri": "../flows/06159210-646b-4c8d-8583-da9b3b95a6c1.xml"}, "exchange direction": "INPUT", "other": {"anies": [{"name": "referenceToUnitGroupDataSet", "value": {"shortDescription": [{"value": "MJ", "lang": "en"}], "type": "unit group data set", "refObjectId": "93a60a57-a3c8-11da-a746-0800200c9a66", "uri": "../unitgroups/93a60a57-a3c8-11da-a746-0800200c9a66.xml"}}, {"value": "516", "module": "A1-A3"}, {"value": "1.88", "module": "A4"}, {"value": "0.225", "module": "A5"}, {"value": "0.176", "module": "C1"}, {"value": "0.942", "module": "C2"}, {"value": "18", "module": "C3"}, {"value": "1.25", "module": "C4"}, {"value": "-104", "module": "D"}]}, "resolvedFlowVersion": "38.00.000", "flowProperties": [], "typeOfFlow": "Other flow", "classification": {"classHierarchy": "Quantities / Environmental quantities / EPD EN 15804 / LCI indicators", "name": "GaBiCategories"}}, {"dataSetInternalID": 7, "referenceToFlowDataSet": {"shortDescription": [{"value": "Use of secondary material (SM)", "lang": "en"}, {"value": "Einsatz von Sekundärstoffen (SM)", "lang": "de"}], "type": "flow data set", "refObjectId": "c6a1f35f-2d09-4f54-8dfb-97e502e1ce92", "uri": "../flows/c6a1f35f-2d09-4f54-8dfb-97e502e1ce92.xml"}, "exchange direction": "INPUT", "other": {"anies": [{"name": "referenceToUnitGroupDataSet", "value": {"shortDescription": [{"value": "kg", "lang": "en"}], "type": "unit group data set", "refObjectId": "ad38d542-3fe9-439d-9b95-2f5f7752acaf", "uri": "../unitgroups/ad38d542-3fe9-439d-9b95-2f5f7752acaf.xml"}}, {"value": "11.4", "module": "A1-A3"}, {"value": "0", "module": "A4"}, {"value": "0", "module": "A5"}, {"value": "0", "module": "C1"}, {"value": "0", "module": "C2"}, {"value": "0", "module": "C3"}, {"value": "0", "module": "C4"}, {"value": "-0.653", "module": "D"}]}, "resolvedFlowVersion": "38.00.000", "flowProperties": [], "typeOfFlow": "Other flow", "classification": {"classHierarchy": "Quantities / Environmental quantities / EPD EN 15804 / LCI indicators", "name": "GaBiCategories"}}, {"dataSetInternalID": 8, "referenceToFlowDataSet": {"shortDescription": [{"value": "Use of renewable secondary fuels (RSF)", "lang": "en"}, {"value": "Erneuerbare Sekundärbrennstoffe (RSF)", "lang": "de"}], "type": "flow data set", "refObjectId": "64333088-a55f-4aa2-9a31-c10b07816787", "uri": "../flows/64333088-a55f-4aa2-9a31-c10b07816787.xml"}, "exchange direction": "INPUT", "other": {"anies": [{"name": "referenceToUnitGroupDataSet", "value": {"shortDescription": [{"value": "MJ", "lang": "en"}], "type": "unit group data set", "refObjectId": "93a60a57-a3c8-11da-a746-0800200c9a66", "uri": "../unitgroups/93a60a57-a3c8-11da-a746-0800200c9a66.xml"}}, {"value": "0", "module": "A1-A3"}, {"value": "0", "module": "A4"}, {"value": "0", "module": "A5"}, {"value": "0", "module": "C1"}, {"value": "0", "module": "C2"}, {"value": "0", "module": "C3"}, {"value": "0", "module": "C4"}, {"value": "0", "module": "D"}]}, "resolvedFlowVersion": "38.00.000", "flowProperties": [], "typeOfFlow": "Other flow", "classification": {"classHierarchy": "Quantities / Environmental quantities / EPD EN 15804 / LCI indicators", "name": "GaBiCategories"}}, {"dataSetInternalID": 9, "referenceToFlowDataSet": {"shortDescription": [{"value": "Use of non renewable secondary fuels (NRSF)", "lang": "en"}, {"value": "Nicht erneuerbare Sekundärbrennstoffe (NRSF)", "lang": "de"}], "type": "flow data set", "refObjectId": "89def144-d39a-4287-b86f-efde453ddcb2", "uri": "../flows/89def144-d39a-4287-b86f-efde453ddcb2.xml"}, "exchange direction": "INPUT", "other": {"anies": [{"name": "referenceToUnitGroupDataSet", "value": {"shortDescription": [{"value": "MJ", "lang": "en"}], "type": "unit group data set", "refObjectId": "93a60a57-a3c8-11da-a746-0800200c9a66", "uri": "../unitgroups/93a60a57-a3c8-11da-a746-0800200c9a66.xml"}}, {"value": "0", "module": "A1-A3"}, {"value": "0", "module": "A4"}, {"value": "0", "module": "A5"}, {"value": "0", "module": "C1"}, {"value": "0", "module": "C2"}, {"value": "0", "module": "C3"}, {"value": "0", "module": "C4"}, {"value": "0", "module": "D"}]}, "resolvedFlowVersion": "38.00.000", "flowProperties": [], "typeOfFlow": "Other flow", "classification": {"classHierarchy": "Quantities / Environmental quantities / EPD EN 15804 / LCI indicators", "name": "GaBiCategories"}}, {"dataSetInternalID": 10, "referenceToFlowDataSet": {"shortDescription": [{"value": "Use of net fresh water (FW)", "lang": "en"}, {"value": "Einsatz von Süßwasserressourcen (FW)", "lang": "de"}], "type": "flow data set", "refObjectId": "3cf952c8-f3a4-461d-8c96-96456ca62246", "uri": "../flows/3cf952c8-f3a4-461d-8c96-96456ca62246.xml"}, "exchange direction": "INPUT", "other": {"anies": [{"name": "referenceToUnitGroupDataSet", "value": {"shortDescription": [{"value": "m^3", "lang": "en"}], "type": "unit group data set", "refObjectId": "cd950537-0a98-4044-9ba7-9f9a68d0a504", "uri": "../unitgroups/cd950537-0a98-4044-9ba7-9f9a68d0a504.xml"}}, {"value": "0.13846", "module": "A1-A3"}, {"value": "0.00015", "module": "A4"}, {"value": "0.00264", "module": "A5"}, {"value": "1.41E-05", "module": "C1"}, {"value": "7.51E-05", "module": "C2"}, {"value": "0.0235", "module": "C3"}, {"value": "0.000317", "module": "C4"}, {"value": "-0.0553", "module": "D"}]}, "resolvedFlowVersion": "38.00.000", "flowProperties": [], "typeOfFlow": "Other flow", "classification": {"classHierarchy": "Quantities / Environmental quantities / EPD EN 15804 / LCI indicators", "name": "GaBiCategories"}}, {"dataSetInternalID": 11, "referenceToFlowDataSet": {"shortDescription": [{"value": "Hazardous waste disposed (HWD)", "lang": "en"}, {"value": "Gefährlicher Abfall zur Deponie (HWD)", "lang": "de"}], "type": "flow data set", "refObjectId": "430f9e0f-59b2-46a0-8e0d-55e0e84948fc", "uri": "../flows/430f9e0f-59b2-46a0-8e0d-55e0e84948fc.xml"}, "exchange direction": "OUTPUT", "other": {"anies": [{"name": "referenceToUnitGroupDataSet", "value": {"shortDescription": [{"value": "kg", "lang": "en"}], "type": "unit group data set", "refObjectId": "ad38d542-3fe9-439d-9b95-2f5f7752acaf", "uri": "../unitgroups/ad38d542-3fe9-439d-9b95-2f5f7752acaf.xml"}}, {"value": "0.000300003386", "module": "A1-A3"}, {"value": "9.97E-12", "module": "A4"}, {"value": "2.17E-11", "module": "A5"}, {"value": "9.33E-13", "module": "C1"}, {"value": "4.99E-12", "module": "C2"}, {"value": "1.4E-09", "module": "C3"}, {"value": "6.41E-11", "module": "C4"}, {"value": "-9.86E-09", "module": "D"}]}, "resolvedFlowVersion": "38.00.000", "flowProperties": [], "typeOfFlow": "Other flow", "classification": {"classHierarchy": "Quantities / Environmental quantities / EPD EN 15804 / LCI indicators", "name": "GaBiCategories"}}, {"dataSetInternalID": 12, "referenceToFlowDataSet": {"shortDescription": [{"value": "Non hazardous waste disposed (NHWD)", "lang": "en"}, {"value": "Entsorgter nicht gefährlicher Abfall (NHWD)", "lang": "de"}], "type": "flow data set", "refObjectId": "b29ef66b-e286-4afa-949f-62f1a7b4d7fa", "uri": "../flows/b29ef66b-e286-4afa-949f-62f1a7b4d7fa.xml"}, "exchange direction": "OUTPUT", "other": {"anies": [{"name": "referenceToUnitGroupDataSet", "value": {"shortDescription": [{"value": "kg", "lang": "en"}], "type": "unit group data set", "refObjectId": "ad38d542-3fe9-439d-9b95-2f5f7752acaf", "uri": "../unitgroups/ad38d542-3fe9-439d-9b95-2f5f7752acaf.xml"}}, {"value": "1.68135", "module": "A1-A3"}, {"value": "0.000307", "module": "A4"}, {"value": "0.0078", "module": "A5"}, {"value": "2.87E-05", "module": "C1"}, {"value": "0.000153", "module": "C2"}, {"value": "6.13", "module": "C3"}, {"value": "6.39", "module": "C4"}, {"value": "-0.764", "module": "D"}]}, "resolvedFlowVersion": "38.00.000", "flowProperties": [], "typeOfFlow": "Other flow", "classification": {"classHierarchy": "Quantities / Environmental quantities / EPD EN 15804 / LCI indicators", "name": "GaBiCategories"}}, {"dataSetInternalID": 13, "referenceToFlowDataSet": {"shortDescription": [{"value": "Radioactive waste disposed (RWD)", "lang": "en"}, {"value": "Entsorgter radioaktiver Abfall (RWD)", "lang": "de"}], "type": "flow data set", "refObjectId": "3449546e-52ad-4b39-b809-9fb77cea8ff6", "uri": "../flows/3449546e-52ad-4b39-b809-9fb77cea8ff6.xml"}, "exchange direction": "OUTPUT", "other": {"anies": [{"name": "referenceToUnitGroupDataSet", "value": {"shortDescription": [{"value": "kg", "lang": "en"}], "type": "unit group data set", "refObjectId": "ad38d542-3fe9-439d-9b95-2f5f7752acaf", "uri": "../unitgroups/ad38d542-3fe9-439d-9b95-2f5f7752acaf.xml"}}, {"value": "0.0220702", "module": "A1-A3"}, {"value": "3.5E-06", "module": "A4"}, {"value": "1.33E-05", "module": "A5"}, {"value": "3.27E-07", "module": "C1"}, {"value": "1.75E-06", "module": "C2"}, {"value": "0.000572", "module": "C3"}, {"value": "1.39E-05", "module": "C4"}, {"value": "-0.00627", "module": "D"}]}, "resolvedFlowVersion": "38.00.000", "flowProperties": [], "typeOfFlow": "Other flow", "classification": {"classHierarchy": "Quantities / Environmental quantities / EPD EN 15804 / LCI indicators", "name": "GaBiCategories"}}, {"dataSetInternalID": 14, "referenceToFlowDataSet": {"shortDescription": [{"value": "Components for re-use (CRU)", "lang": "en"}, {"value": "Komponenten für die Wiederverwendung (CRU)", "lang": "de"}], "type": "flow data set", "refObjectId": "a2b32f97-3fc7-4af2-b209-525bc6426f33", "uri": "../flows/a2b32f97-3fc7-4af2-b209-525bc6426f33.xml"}, "exchange direction": "OUTPUT", "other": {"anies": [{"name": "referenceToUnitGroupDataSet", "value": {"shortDescription": [{"value": "kg", "lang": "en"}], "type": "unit group data set", "refObjectId": "ad38d542-3fe9-439d-9b95-2f5f7752acaf", "uri": "../unitgroups/ad38d542-3fe9-439d-9b95-2f5f7752acaf.xml"}}, {"value": "0", "module": "A1-A3"}, {"value": "0", "module": "A4"}, {"value": "0", "module": "A5"}, {"value": "0", "module": "C1"}, {"value": "0", "module": "C2"}, {"value": "0", "module": "C3"}, {"value": "0", "module": "C4"}, {"value": "0", "module": "D"}]}, "resolvedFlowVersion": "38.00.000", "flowProperties": [], "typeOfFlow": "Other flow", "classification": {"classHierarchy": "Quantities / Environmental quantities / EPD EN 15804 / LCI indicators", "name": "GaBiCategories"}}, {"dataSetInternalID": 15, "referenceToFlowDataSet": {"shortDescription": [{"value": "Materials for recycling (MFR)", "lang": "en"}, {"value": "Stoffe zum Recycling (MFR)", "lang": "de"}], "type": "flow data set", "refObjectId": "d7fe48a5-4103-49c8-9aae-b0b5dfdbd6ae", "uri": "../flows/d7fe48a5-4103-49c8-9aae-b0b5dfdbd6ae.xml"}, "exchange direction": "OUTPUT", "other": {"anies": [{"name": "referenceToUnitGroupDataSet", "value": {"shortDescription": [{"value": "kg", "lang": "en"}], "type": "unit group data set", "refObjectId": "ad38d542-3fe9-439d-9b95-2f5f7752acaf", "uri": "../unitgroups/ad38d542-3fe9-439d-9b95-2f5f7752acaf.xml"}}, {"value": "0.00617", "module": "A1-A3"}, {"value": "0", "module": "A4"}, {"value": "0", "module": "A5"}, {"value": "0", "module": "C1"}, {"value": "0", "module": "C2"}, {"value": "10.7", "module": "C3"}, {"value": "0", "module": "C4"}, {"value": "0", "module": "D"}]}, "resolvedFlowVersion": "38.00.000", "flowProperties": [], "typeOfFlow": "Other flow", "classification": {"classHierarchy": "Quantities / Environmental quantities / EPD EN 15804 / LCI indicators", "name": "GaBiCategories"}}, {"dataSetInternalID": 16, "referenceToFlowDataSet": {"shortDescription": [{"value": "Materials for energy recovery (MER)", "lang": "en"}, {"value": "Stoffe für die Energierückgewinnung (MER)", "lang": "de"}], "type": "flow data set", "refObjectId": "59a9181c-3aaf-46ee-8b13-2b3723b6e447", "uri": "../flows/59a9181c-3aaf-46ee-8b13-2b3723b6e447.xml"}, "exchange direction": "OUTPUT", "other": {"anies": [{"name": "referenceToUnitGroupDataSet", "value": {"shortDescription": [{"value": "kg", "lang": "en"}], "type": "unit group data set", "refObjectId": "ad38d542-3fe9-439d-9b95-2f5f7752acaf", "uri": "../unitgroups/ad38d542-3fe9-439d-9b95-2f5f7752acaf.xml"}}, {"value": "0", "module": "A1-A3"}, {"value": "0", "module": "A4"}, {"value": "0", "module": "A5"}, {"value": "0", "module": "C1"}, {"value": "0", "module": "C2"}, {"value": "0", "module": "C3"}, {"value": "0", "module": "C4"}, {"value": "0", "module": "D"}]}, "resolvedFlowVersion": "38.00.000", "flowProperties": [], "typeOfFlow": "Other flow", "classification": {"classHierarchy": "Quantities / Environmental quantities / EPD EN 15804 / LCI indicators", "name": "GaBiCategories"}}, {"dataSetInternalID": 17, "referenceToFlowDataSet": {"shortDescription": [{"value": "Exported electrical energy (EEE)", "lang": "en"}, {"value": "Exportierte elektrische Energie (EEE)", "lang": "de"}], "type": "flow data set", "refObjectId": "4da0c987-2b76-40d6-9e9e-82a017aaaf29", "uri": "../flows/4da0c987-2b76-40d6-9e9e-82a017aaaf29.xml"}, "exchange direction": "OUTPUT", "other": {"anies": [{"name": "referenceToUnitGroupDataSet", "value": {"shortDescription": [{"value": "MJ", "lang": "en"}], "type": "unit group data set", "refObjectId": "93a60a57-a3c8-11da-a746-0800200c9a66", "uri": "../unitgroups/93a60a57-a3c8-11da-a746-0800200c9a66.xml"}}, {"value": "0", "module": "A1-A3"}, {"value": "0", "module": "A4"}, {"value": "1.57", "module": "A5"}, {"value": "0", "module": "C1"}, {"value": "0", "module": "C2"}, {"value": "13.3", "module": "C3"}, {"value": "0", "module": "C4"}, {"value": "0", "module": "D"}]}, "resolvedFlowVersion": "38.00.000", "flowProperties": [], "typeOfFlow": "Other flow", "classification": {"classHierarchy": "Quantities / Environmental quantities / EPD EN 15804 / LCI indicators", "name": "GaBiCategories"}}, {"dataSetInternalID": 18, "referenceToFlowDataSet": {"shortDescription": [{"value": "Exported thermal energy (EET)", "lang": "en"}, {"value": "Exportierte thermische Energie (EET)", "lang": "de"}], "type": "flow data set", "refObjectId": "98daf38a-7a79-46d3-9a37-2b7bd0955810", "uri": "../flows/98daf38a-7a79-46d3-9a37-2b7bd0955810.xml"}, "exchange direction": "OUTPUT", "other": {"anies": [{"name": "referenceToUnitGroupDataSet", "value": {"shortDescription": [{"value": "MJ", "lang": "en"}], "type": "unit group data set", "refObjectId": "93a60a57-a3c8-11da-a746-0800200c9a66", "uri": "../unitgroups/93a60a57-a3c8-11da-a746-0800200c9a66.xml"}}, {"value": "0", "module": "A1-A3"}, {"value": "0", "module": "A4"}, {"value": "2.82", "module": "A5"}, {"value": "0", "module": "C1"}, {"value": "0", "module": "C2"}, {"value": "24.2", "module": "C3"}, {"value": "0", "module": "C4"}, {"value": "0", "module": "D"}]}, "resolvedFlowVersion": "38.00.000", "flowProperties": [], "typeOfFlow": "Other flow", "classification": {"classHierarchy": "Quantities / Environmental quantities / EPD EN 15804 / LCI indicators", "name": "GaBiCategories"}}]}, "LCIAResults": {"LCIAResult": [{"referenceToLCIAMethodDataSet": {"shortDescription": [{"value": "Global Warming Potential total (GWP-total)", "lang": "en"}, {"value": "Globales Erwärmungspotenzial total (GWP-total)", "lang": "de"}], "type": "LCIA method data set", "refObjectId": "6a37f984-a4b3-458a-a20a-64418c145fa2", "uri": "../lciamethods/6a37f984-a4b3-458a-a20a-64418c145fa2.xml"}, "other": {"anies": [{"name": "referenceToUnitGroupDataSet", "value": {"shortDescription": [{"value": "kg CO_(2) eq", "lang": "en"}], "type": "unit group data set", "refObjectId": "1ebf3012-d0db-4de2-aefd-ef30cedb0be1", "uri": "../unitgroups/1ebf3012-d0db-4de2-aefd-ef30cedb0be1.xml"}}, {"value": "28.84", "module": "A1-A3"}, {"value": "0.144", "module": "A4"}, {"value": "1.03", "module": "A5"}, {"value": "0.0139901", "module": "C1"}, {"value": "0.0729", "module": "C2"}, {"value": "11.5", "module": "C3"}, {"value": "0.0926", "module": "C4"}, {"value": "-6.18", "module": "D"}]}}, {"referenceToLCIAMethodDataSet": {"shortDescription": [{"value": "Global Warming Potential fossil fuels (GWP-fossil)", "lang": "en"}, {"value": "Globales Erwärmungspotenzial fossil (GWP-fossil)", "lang": "de"}], "type": "LCIA method data set", "refObjectId": "5f635281-343e-44fb-83df-1971b155e6b6", "uri": "../lciamethods/5f635281-343e-44fb-83df-1971b155e6b6.xml"}, "other": {"anies": [{"name": "referenceToUnitGroupDataSet", "value": {"shortDescription": [{"value": "kg CO_(2) eq", "lang": "en"}], "type": "unit group data set", "refObjectId": "1ebf3012-d0db-4de2-aefd-ef30cedb0be1", "uri": "../unitgroups/1ebf3012-d0db-4de2-aefd-ef30cedb0be1.xml"}}, {"value": "29.75", "module": "A1-A3"}, {"value": "0.143", "module": "A4"}, {"value": "0.0155", "module": "A5"}, {"value": "0.0139", "module": "C1"}, {"value": "0.0713", "module": "C2"}, {"value": "11.5", "module": "C3"}, {"value": "0.0952", "module": "C4"}, {"value": "-6.2", "module": "D"}]}}, {"referenceToLCIAMethodDataSet": {"shortDescription": [{"value": "Global Warming Potential biogenic (GWP-biogenic)", "lang": "en"}, {"value": "Globales Erwärmungspotenzial biogen (GWP-biogenic)", "lang": "de"}], "type": "LCIA method data set", "refObjectId": "2356e1ab-0185-4db5-86e5-16de51c7485c", "uri": "../lciamethods/2356e1ab-0185-4db5-86e5-16de51c7485c.xml"}, "other": {"anies": [{"name": "referenceToUnitGroupDataSet", "value": {"shortDescription": [{"value": "kg CO_(2) eq", "lang": "en"}], "type": "unit group data set", "refObjectId": "1ebf3012-d0db-4de2-aefd-ef30cedb0be1", "uri": "../unitgroups/1ebf3012-d0db-4de2-aefd-ef30cedb0be1.xml"}}, {"value": "-0.8912", "module": "A1-A3"}, {"value": "0.000464", "module": "A4"}, {"value": "1.02", "module": "A5"}, {"value": "0", "module": "C1"}, {"value": "0.00116", "module": "C2"}, {"value": "0.00151", "module": "C3"}, {"value": "-0.00282", "module": "C4"}, {"value": "0.0162", "module": "D"}]}}, {"referenceToLCIAMethodDataSet": {"shortDescription": [{"value": "Global Warming Potential luluc (GWP-luluc)", "lang": "en"}, {"value": "Globales Erwärmungspotenzial luluc (GWP-luluc)", "lang": "de"}], "type": "LCIA method data set", "refObjectId": "4331bbdb-978a-490d-8707-eeb047f01a55", "uri": "../lciamethods/4331bbdb-978a-490d-8707-eeb047f01a55.xml"}, "other": {"anies": [{"name": "referenceToUnitGroupDataSet", "value": {"shortDescription": [{"value": "kg CO_(2) eq", "lang": "en"}], "type": "unit group data set", "refObjectId": "1ebf3012-d0db-4de2-aefd-ef30cedb0be1", "uri": "../unitgroups/1ebf3012-d0db-4de2-aefd-ef30cedb0be1.xml"}}, {"value": "0.018034", "module": "A1-A3"}, {"value": "0.000963", "module": "A4"}, {"value": "2.06E-06", "module": "A5"}, {"value": "9.01E-05", "module": "C1"}, {"value": "0.000482", "module": "C2"}, {"value": "0.000776", "module": "C3"}, {"value": "0.000176", "module": "C4"}, {"value": "-0.00372", "module": "D"}]}}, {"referenceToLCIAMethodDataSet": {"shortDescription": [{"value": "Depletion potential of the stratospheric ozone layer (ODP)", "lang": "en"}, {"value": "Abbau Potential der stratosphärischen Ozonschicht (ODP)", "lang": "de"}], "type": "LCIA method data set", "refObjectId": "b5c629d6-def3-11e6-bf01-fe55135034f3", "uri": "../lciamethods/b5c629d6-def3-11e6-bf01-fe55135034f3.xml"}, "other": {"anies": [{"name": "referenceToUnitGroupDataSet", "value": {"shortDescription": [{"value": "kg CFC11 eq", "lang": "en"}], "type": "unit group data set", "refObjectId": "d9e957c9-7309-4474-bf3a-7777df6c4e5b", "uri": "../unitgroups/d9e957c9-7309-4474-bf3a-7777df6c4e5b.xml"}}, {"value": "7.04951E-10", "module": "A1-A3"}, {"value": "1.4E-14", "module": "A4"}, {"value": "8.15E-14", "module": "A5"}, {"value": "1.31E-15", "module": "C1"}, {"value": "7.02E-15", "module": "C2"}, {"value": "9.66E-12", "module": "C3"}, {"value": "2.24E-13", "module": "C4"}, {"value": "-2.3E-11", "module": "D"}]}}, {"referenceToLCIAMethodDataSet": {"shortDescription": [{"value": "Acidification potential of land and water (AP)", "lang": "en"}, {"value": "Versauerungspotenzial von Boden und Wasser (AP)", "lang": "de"}], "type": "LCIA method data set", "refObjectId": "b5c611c6-def3-11e6-bf01-fe55135034f3", "uri": "../lciamethods/b5c611c6-def3-11e6-bf01-fe55135034f3.xml"}, "other": {"anies": [{"name": "referenceToUnitGroupDataSet", "value": {"shortDescription": [{"value": "mol H^(+) eq", "lang": "en"}], "type": "unit group data set", "refObjectId": "42e089ac-92bf-4bf2-8ca1-5fc40d18f2ed", "uri": "../unitgroups/42e089ac-92bf-4bf2-8ca1-5fc40d18f2ed.xml"}}, {"value": "0.10076", "module": "A1-A3"}, {"value": "0.00016", "module": "A4"}, {"value": "0.000154", "module": "A5"}, {"value": "6.73E-05", "module": "C1"}, {"value": "8.02E-05", "module": "C2"}, {"value": "0.0027", "module": "C3"}, {"value": "0.000675", "module": "C4"}, {"value": "-0.0307", "module": "D"}]}}, {"referenceToLCIAMethodDataSet": {"shortDescription": [{"value": "Eutrophication potential aquatic freshwater (EP-freshwater)", "lang": "en"}, {"value": "Eutrophierungspotenzial Süßwasser (EP-freshwater)", "lang": "de"}], "type": "LCIA method data set", "refObjectId": "b53ec18f-7377-4ad3-86eb-cc3f4f276b2b", "uri": "../lciamethods/b53ec18f-7377-4ad3-86eb-cc3f4f276b2b.xml"}, "other": {"anies": [{"name": "referenceToUnitGroupDataSet", "value": {"shortDescription": [{"value": "kg P eq", "lang": "en"}], "type": "unit group data set", "refObjectId": "0429039d-a61d-4590-ba67-aa4a20a810a1", "uri": "../unitgroups/0429039d-a61d-4590-ba67-aa4a20a810a1.xml"}}, {"value": "5.252E-05", "module": "A1-A3"}, {"value": "5.11E-07", "module": "A4"}, {"value": "1.94E-08", "module": "A5"}, {"value": "4.78E-08", "module": "C1"}, {"value": "2.55E-07", "module": "C2"}, {"value": "2.46E-06", "module": "C3"}, {"value": "1.61E-07", "module": "C4"}, {"value": "-3.09E-06", "module": "D"}]}}, {"referenceToLCIAMethodDataSet": {"shortDescription": [{"value": "Eutrophication potential aquatic marine (EP-marine)", "lang": "en"}, {"value": "Eutrophierungspotenzial Salzwasser (EP-marine)", "lang": "de"}], "type": "LCIA method data set", "refObjectId": "b5c619fa-def3-11e6-bf01-fe55135034f3", "uri": "../lciamethods/b5c619fa-def3-11e6-bf01-fe55135034f3.xml"}, "other": {"anies": [{"name": "referenceToUnitGroupDataSet", "value": {"shortDescription": [{"value": "kg N eq", "lang": "en"}], "type": "unit group data set", "refObjectId": "d05bb823-ecdf-4686-8c40-bf1d9257859f", "uri": "../unitgroups/d05bb823-ecdf-4686-8c40-bf1d9257859f.xml"}}, {"value": "0.016957", "module": "A1-A3"}, {"value": "5.18E-05", "module": "A4"}, {"value": "5.03E-05", "module": "A5"}, {"value": "3.15E-05", "module": "C1"}, {"value": "2.59E-05", "module": "C2"}, {"value": "0.000867", "module": "C3"}, {"value": "0.000173", "module": "C4"}, {"value": "-0.00371", "module": "D"}]}}, {"referenceToLCIAMethodDataSet": {"shortDescription": [{"value": "Eutrophication potential terrestrial (EP-terrestrial)", "lang": "en"}, {"value": "Eutrophierungspotenzial Land (EP-terrestrial)", "lang": "de"}], "type": "LCIA method data set", "refObjectId": "b5c614d2-def3-11e6-bf01-fe55135034f3", "uri": "../lciamethods/b5c614d2-def3-11e6-bf01-fe55135034f3.xml"}, "other": {"anies": [{"name": "referenceToUnitGroupDataSet", "value": {"shortDescription": [{"value": "mol N eq", "lang": "en"}], "type": "unit group data set", "refObjectId": "71b4d617-0ec9-4d3f-b65e-e438940c2401", "uri": "../unitgroups/71b4d617-0ec9-4d3f-b65e-e438940c2401.xml"}}, {"value": "0.22635", "module": "A1-A3"}, {"value": "0.00062", "module": "A4"}, {"value": "0.000731", "module": "A5"}, {"value": "0.000349", "module": "C1"}, {"value": "0.00031", "module": "C2"}, {"value": "0.0111", "module": "C3"}, {"value": "0.0019", "module": "C4"}, {"value": "-0.043", "module": "D"}]}}, {"referenceToLCIAMethodDataSet": {"shortDescription": [{"value": "Formation potential of tropospheric ozone photochemical oxidants (POCP)", "lang": "en"}, {"value": "Bildungspotential für troposphärisches Ozon (POCP)", "lang": "de"}], "type": "LCIA method data set", "refObjectId": "b5c610fe-def3-11e6-bf01-fe55135034f3", "uri": "../lciamethods/b5c610fe-def3-11e6-bf01-fe55135034f3.xml"}, "other": {"anies": [{"name": "referenceToUnitGroupDataSet", "value": {"shortDescription": [{"value": "kg NMVOC eq", "lang": "en"}], "type": "unit group data set", "refObjectId": "d27c25f8-fbc1-44c6-b47b-4adbae4199c6", "uri": "../unitgroups/d27c25f8-fbc1-44c6-b47b-4adbae4199c6.xml"}}, {"value": "0.06214", "module": "A1-A3"}, {"value": "0.000138", "module": "A4"}, {"value": "0.000136", "module": "A5"}, {"value": "8.8E-05", "module": "C1"}, {"value": "6.9E-05", "module": "C2"}, {"value": "0.00251", "module": "C3"}, {"value": "0.000525", "module": "C4"}, {"value": "-0.0107", "module": "D"}]}}, {"referenceToLCIAMethodDataSet": {"shortDescription": [{"value": "Abiotic depletion potential for non fossil resources (ADPE)", "lang": "en"}, {"value": "Potenzial für den abiotischen Abbau nicht fossiler Ressourcen (ADPE)", "lang": "de"}], "type": "LCIA method data set", "refObjectId": "b2ad6494-c78d-11e6-9d9d-cec0c932ce01", "uri": "../lciamethods/b2ad6494-c78d-11e6-9d9d-cec0c932ce01.xml"}, "other": {"anies": [{"name": "referenceToUnitGroupDataSet", "value": {"shortDescription": [{"value": "kg Sb eq", "lang": "en"}], "type": "unit group data set", "refObjectId": "54ccd2d9-a32a-4fc2-923d-f2c8c93e89d4", "uri": "../unitgroups/54ccd2d9-a32a-4fc2-923d-f2c8c93e89d4.xml"}}, {"value": "0.000261273", "module": "A1-A3"}, {"value": "1.44E-08", "module": "A4"}, {"value": "1.99E-09", "module": "A5"}, {"value": "1.35E-09", "module": "C1"}, {"value": "7.21E-09", "module": "C2"}, {"value": "2.37E-07", "module": "C3"}, {"value": "9.76E-09", "module": "C4"}, {"value": "-0.000134", "module": "D"}]}}, {"referenceToLCIAMethodDataSet": {"shortDescription": [{"value": "Abiotic depletion potential for fossil resources (ADPF)", "lang": "en"}, {"value": "Potenzial für den abiotischen Abbau fossiler Brennstoffe (ADPF)", "lang": "de"}], "type": "LCIA method data set", "refObjectId": "b2ad6110-c78d-11e6-9d9d-cec0c932ce01", "uri": "../lciamethods/b2ad6110-c78d-11e6-9d9d-cec0c932ce01.xml"}, "other": {"anies": [{"name": "referenceToUnitGroupDataSet", "value": {"shortDescription": [{"value": "MJ", "lang": "en"}], "type": "unit group data set", "refObjectId": "93a60a57-a3c8-11da-a746-0800200c9a66", "uri": "../unitgroups/93a60a57-a3c8-11da-a746-0800200c9a66.xml"}}, {"value": "514.9", "module": "A1-A3"}, {"value": "1.88", "module": "A4"}, {"value": "0.225", "module": "A5"}, {"value": "0.176", "module": "C1"}, {"value": "0.938", "module": "C2"}, {"value": "18", "module": "C3"}, {"value": "1.25", "module": "C4"}, {"value": "-103", "module": "D"}]}}, {"referenceToLCIAMethodDataSet": {"shortDescription": [{"value": "Water use (WDP)", "lang": "en"}, {"value": "Wassernutzung (WDP)", "lang": "de"}], "type": "LCIA method data set", "refObjectId": "b2ad66ce-c78d-11e6-9d9d-cec0c932ce01", "uri": "../lciamethods/b2ad66ce-c78d-11e6-9d9d-cec0c932ce01.xml"}, "other": {"anies": [{"name": "referenceToUnitGroupDataSet", "value": {"shortDescription": [{"value": "m^(3) world eq deprived", "lang": "en"}], "type": "unit group data set", "refObjectId": "6ae2df01-888e-46c8-b17d-49fa3869b476", "uri": "../unitgroups/6ae2df01-888e-46c8-b17d-49fa3869b476.xml"}}, {"value": "3.2934", "module": "A1-A3"}, {"value": "0.0016", "module": "A4"}, {"value": "0.113", "module": "A5"}, {"value": "0.00015", "module": "C1"}, {"value": "0.0008", "module": "C2"}, {"value": "0.913", "module": "C3"}, {"value": "0.0104", "module": "C4"}, {"value": "-1.48", "module": "D"}]}}, {"referenceToLCIAMethodDataSet": {"shortDescription": [{"value": "Incidence of disease due to PM emissions (PM)", "lang": "en"}, {"value": "Auftreten von Krankheiten aufgrund von Feinstaubemissionen (PM)", "lang": "de"}], "type": "LCIA method data set", "refObjectId": "b5c602c6-def3-11e6-bf01-fe55135034f3", "uri": "../lciamethods/b5c602c6-def3-11e6-bf01-fe55135034f3.xml"}, "other": {"anies": [{"name": "referenceToUnitGroupDataSet", "value": {"shortDescription": [{"value": "Disease incidence", "lang": "en"}], "type": "unit group data set", "refObjectId": "3883559b-648f-4afc-8ba2-0bd24f3affa3", "uri": "../unitgroups/3883559b-648f-4afc-8ba2-0bd24f3affa3.xml"}}, {"value": "1.2951E-06", "module": "A1-A3"}, {"value": "1.1E-09", "module": "A4"}, {"value": "7.55E-10", "module": "A5"}, {"value": "7.64E-10", "module": "C1"}, {"value": "5.5E-10", "module": "C2"}, {"value": "6.67E-08", "module": "C3"}, {"value": "8.31E-09", "module": "C4"}, {"value": "-4.64E-07", "module": "D"}]}}, {"referenceToLCIAMethodDataSet": {"shortDescription": [{"value": "Human exposure efficiency relative to U235 (IR)", "lang": "en"}, {"value": "Wirkung durch Exposition des Menschen mit U235 (IR)", "lang": "de"}], "type": "LCIA method data set", "refObjectId": "b5c632be-def3-11e6-bf01-fe55135034f3", "uri": "../lciamethods/b5c632be-def3-11e6-bf01-fe55135034f3.xml"}, "other": {"anies": [{"name": "referenceToUnitGroupDataSet", "value": {"shortDescription": [{"value": "kBq U235 eq", "lang": "en"}], "type": "unit group data set", "refObjectId": "456b05bf-1415-44a9-9993-02452f554c09", "uri": "../unitgroups/456b05bf-1415-44a9-9993-02452f554c09.xml"}}, {"value": "3.12356", "module": "A1-A3"}, {"value": "0.000528", "module": "A4"}, {"value": "0.00218", "module": "A5"}, {"value": "4.94E-05", "module": "C1"}, {"value": "0.000264", "module": "C2"}, {"value": "0.0637", "module": "C3"}, {"value": "0.00154", "module": "C4"}, {"value": "-0.979", "module": "D"}]}}, {"referenceToLCIAMethodDataSet": {"shortDescription": [{"value": "Comparative toxic unit for ecosystems (ETP-fw)", "lang": "en"}, {"value": "Toxizitätsvergleichseinheit für Ökosysteme (ETP-fw)", "lang": "de"}], "type": "LCIA method data set", "refObjectId": "ee1082d1-b0f7-43ca-a1f0-21e2a4a74511", "uri": "../lciamethods/ee1082d1-b0f7-43ca-a1f0-21e2a4a74511.xml"}, "other": {"anies": [{"name": "referenceToUnitGroupDataSet", "value": {"shortDescription": [{"value": "CTUe", "lang": "en"}], "type": "unit group data set", "refObjectId": "aa959ded-f1eb-4efb-9c5c-2d60be36b3e6", "uri": "../unitgroups/aa959ded-f1eb-4efb-9c5c-2d60be36b3e6.xml"}}, {"value": "244", "module": "A1-A3"}, {"value": "1.33", "module": "A4"}, {"value": "0.0992", "module": "A5"}, {"value": "0.124", "module": "C1"}, {"value": "0.665", "module": "C2"}, {"value": "15", "module": "C3"}, {"value": "0.699", "module": "C4"}, {"value": "-47.8", "module": "D"}]}}, {"referenceToLCIAMethodDataSet": {"shortDescription": [{"value": "Comparative toxic unit for humans (carcinogenic) (HTP-c)", "lang": "en"}, {"value": "Toxizitätsvergleichseinheit für Menschen (krebserregend) (HTP-c)", "lang": "de"}], "type": "LCIA method data set", "refObjectId": "2299222a-bbd8-474f-9d4f-4dd1f18aea7c", "uri": "../lciamethods/2299222a-bbd8-474f-9d4f-4dd1f18aea7c.xml"}, "other": {"anies": [{"name": "referenceToUnitGroupDataSet", "value": {"shortDescription": [{"value": "CTUh", "lang": "en"}], "type": "unit group data set", "refObjectId": "d4c9523e-2d7e-49fd-8469-998f547d3a70", "uri": "../unitgroups/d4c9523e-2d7e-49fd-8469-998f547d3a70.xml"}}, {"value": "2.790526E-06", "module": "A1-A3"}, {"value": "2.74E-11", "module": "A4"}, {"value": "6.76E-12", "module": "A5"}, {"value": "2.56E-12", "module": "C1"}, {"value": "1.37E-11", "module": "C2"}, {"value": "6.05E-10", "module": "C3"}, {"value": "1.07E-10", "module": "C4"}, {"value": "-8.68E-09", "module": "D"}]}}, {"referenceToLCIAMethodDataSet": {"shortDescription": [{"value": "Comparative toxic unit for humans (noncarcinogenic) (HTP-nc)", "lang": "en"}, {"value": "Toxizitätsvergleichseinheit für Menschen (nicht krebserregend) (HTP-nc)", "lang": "de"}], "type": "LCIA method data set", "refObjectId": "3af763a5-b7a1-48c9-9cee-1f223481fcef", "uri": "../lciamethods/3af763a5-b7a1-48c9-9cee-1f223481fcef.xml"}, "other": {"anies": [{"name": "referenceToUnitGroupDataSet", "value": {"shortDescription": [{"value": "CTUh", "lang": "en"}], "type": "unit group data set", "refObjectId": "d4c9523e-2d7e-49fd-8469-998f547d3a70", "uri": "../unitgroups/d4c9523e-2d7e-49fd-8469-998f547d3a70.xml"}}, {"value": "9.549E-07", "module": "A1-A3"}, {"value": "1.48E-09", "module": "A4"}, {"value": "2.36E-10", "module": "A5"}, {"value": "1.61E-10", "module": "C1"}, {"value": "7.42E-10", "module": "C2"}, {"value": "6.38E-08", "module": "C3"}, {"value": "1.18E-08", "module": "C4"}, {"value": "-1.46E-08", "module": "D"}]}}, {"referenceToLCIAMethodDataSet": {"shortDescription": [{"value": "Soil quality index (SQP)", "lang": "en"}, {"value": "Bodenqualitätsindex (SQP)", "lang": "de"}], "type": "LCIA method data set", "refObjectId": "b2ad6890-c78d-11e6-9d9d-cec0c932ce01", "uri": "../lciamethods/b2ad6890-c78d-11e6-9d9d-cec0c932ce01.xml"}, "other": {"anies": [{"name": "referenceToUnitGroupDataSet", "value": {"shortDescription": [{"value": "SQP", "lang": "en"}], "type": "unit group data set", "refObjectId": "f130951c-e67f-4f7f-8dd4-665de3974e18", "uri": "../unitgroups/f130951c-e67f-4f7f-8dd4-665de3974e18.xml"}}, {"value": "353.36", "module": "A1-A3"}, {"value": "0.794", "module": "A4"}, {"value": "0.0666", "module": "A5"}, {"value": "0.0743", "module": "C1"}, {"value": "0.397", "module": "C2"}, {"value": "4.13", "module": "C3"}, {"value": "0.259", "module": "C4"}, {"value": "-9.84", "module": "D"}]}}]}, "otherAttributes": {"{http://www.indata.network/EPD/2019}epd-version": "1.2"}, "version": "1.1", "locations": "../ILCDLocations.xml"}