{"processInformation": {"dataSetInformation": {"UUID": "c6168528-57b9-409a-b94d-a124b438d650", "name": {"baseName": [{"value": "Monarflex Necoseal (Radon Barrier, BMI Group Holdings UK Limited)", "lang": "en"}, {"value": "Monarflex Necoseal (Radon Barriere, BMI Group Holdings UK Limited)", "lang": "de"}]}, "synonyms": [{"value": "Monarflex Necoseal (BMI Group Holdings UK Limited)", "lang": "en"}], "classificationInformation": {"classification": [{"class": [{"value": "Kunststoffe", "level": 0, "classId": "6"}, {"value": "Folien und Vliese", "level": 1, "classId": "6.6"}, {"value": "Unterspannbahn", "level": 2, "classId": "6.6.01"}], "name": "OEKOBAU.DAT"}]}, "generalComment": [{"value": "The owner of this EPD shall be liable for the underlying information and evidence. The programme operator Kiwa-Ecobility Experts shall not be liable with respect to manufacturer data, life cycle assessment data and evidence. This is a Cradle to gate with options, modules C1-C4 and module D EPD.", "lang": "en"}], "other": {"anies": [{"scenario": [{"description": [{"value": "For areas where accurate data was not available, such as transport or end-of-life scenarios, we used default values like for transport Lorry (Truck), unspecified (default) | market group for (GLO), EcoInvent 3.6 (2019) and for eol polyolefines (i.a. pe,pp) (i.a. pipes, foils) (NMD ID 57) for the main product and different eols for the packaging.", "lang": "en"}], "name": "Standard Scenario", "default": true}]}, "<ns11:modules xmlns:ns11=\"http://openlca.org/epd_ilcd\" xmlns=\"http://lca.jrc.it/ILCD/Process\" xmlns:c=\"http://lca.jrc.it/ILCD/Contact\" xmlns:common=\"http://lca.jrc.it/ILCD/Common\" xmlns:epd=\"http://www.iai.kit.edu/EPD/2013\" xmlns:epd2=\"http://www.indata.network/EPD/2019\" xmlns:f=\"http://lca.jrc.it/ILCD/Flow\" xmlns:fp=\"http://lca.jrc.it/ILCD/FlowProperty\" xmlns:m=\"http://lca.jrc.it/ILCD/LCIAMethod\" xmlns:s=\"http://lca.jrc.it/ILCD/Source\" xmlns:u=\"http://lca.jrc.it/ILCD/UnitGroup\" name=\"A1\" scenario=\"Standard Scenario\"/>", "<ns11:modules xmlns:ns11=\"http://openlca.org/epd_ilcd\" xmlns=\"http://lca.jrc.it/ILCD/Process\" xmlns:c=\"http://lca.jrc.it/ILCD/Contact\" xmlns:common=\"http://lca.jrc.it/ILCD/Common\" xmlns:epd=\"http://www.iai.kit.edu/EPD/2013\" xmlns:epd2=\"http://www.indata.network/EPD/2019\" xmlns:f=\"http://lca.jrc.it/ILCD/Flow\" xmlns:fp=\"http://lca.jrc.it/ILCD/FlowProperty\" xmlns:m=\"http://lca.jrc.it/ILCD/LCIAMethod\" xmlns:s=\"http://lca.jrc.it/ILCD/Source\" xmlns:u=\"http://lca.jrc.it/ILCD/UnitGroup\" name=\"A1-A3\" scenario=\"Standard Scenario\"/>", "<ns11:modules xmlns:ns11=\"http://openlca.org/epd_ilcd\" xmlns=\"http://lca.jrc.it/ILCD/Process\" xmlns:c=\"http://lca.jrc.it/ILCD/Contact\" xmlns:common=\"http://lca.jrc.it/ILCD/Common\" xmlns:epd=\"http://www.iai.kit.edu/EPD/2013\" xmlns:epd2=\"http://www.indata.network/EPD/2019\" xmlns:f=\"http://lca.jrc.it/ILCD/Flow\" xmlns:fp=\"http://lca.jrc.it/ILCD/FlowProperty\" xmlns:m=\"http://lca.jrc.it/ILCD/LCIAMethod\" xmlns:s=\"http://lca.jrc.it/ILCD/Source\" xmlns:u=\"http://lca.jrc.it/ILCD/UnitGroup\" name=\"A2\" scenario=\"Standard Scenario\"/>", "<ns11:modules xmlns:ns11=\"http://openlca.org/epd_ilcd\" xmlns=\"http://lca.jrc.it/ILCD/Process\" xmlns:c=\"http://lca.jrc.it/ILCD/Contact\" xmlns:common=\"http://lca.jrc.it/ILCD/Common\" xmlns:epd=\"http://www.iai.kit.edu/EPD/2013\" xmlns:epd2=\"http://www.indata.network/EPD/2019\" xmlns:f=\"http://lca.jrc.it/ILCD/Flow\" xmlns:fp=\"http://lca.jrc.it/ILCD/FlowProperty\" xmlns:m=\"http://lca.jrc.it/ILCD/LCIAMethod\" xmlns:s=\"http://lca.jrc.it/ILCD/Source\" xmlns:u=\"http://lca.jrc.it/ILCD/UnitGroup\" name=\"A3\" scenario=\"Standard Scenario\"/>", "<ns11:modules xmlns:ns11=\"http://openlca.org/epd_ilcd\" xmlns=\"http://lca.jrc.it/ILCD/Process\" xmlns:c=\"http://lca.jrc.it/ILCD/Contact\" xmlns:common=\"http://lca.jrc.it/ILCD/Common\" xmlns:epd=\"http://www.iai.kit.edu/EPD/2013\" xmlns:epd2=\"http://www.indata.network/EPD/2019\" xmlns:f=\"http://lca.jrc.it/ILCD/Flow\" xmlns:fp=\"http://lca.jrc.it/ILCD/FlowProperty\" xmlns:m=\"http://lca.jrc.it/ILCD/LCIAMethod\" xmlns:s=\"http://lca.jrc.it/ILCD/Source\" xmlns:u=\"http://lca.jrc.it/ILCD/UnitGroup\" name=\"A4\" scenario=\"Standard Scenario\"/>", "<ns11:modules xmlns:ns11=\"http://openlca.org/epd_ilcd\" xmlns=\"http://lca.jrc.it/ILCD/Process\" xmlns:c=\"http://lca.jrc.it/ILCD/Contact\" xmlns:common=\"http://lca.jrc.it/ILCD/Common\" xmlns:epd=\"http://www.iai.kit.edu/EPD/2013\" xmlns:epd2=\"http://www.indata.network/EPD/2019\" xmlns:f=\"http://lca.jrc.it/ILCD/Flow\" xmlns:fp=\"http://lca.jrc.it/ILCD/FlowProperty\" xmlns:m=\"http://lca.jrc.it/ILCD/LCIAMethod\" xmlns:s=\"http://lca.jrc.it/ILCD/Source\" xmlns:u=\"http://lca.jrc.it/ILCD/UnitGroup\" name=\"A5\" scenario=\"Standard Scenario\"/>", "<ns11:modules xmlns:ns11=\"http://openlca.org/epd_ilcd\" xmlns=\"http://lca.jrc.it/ILCD/Process\" xmlns:c=\"http://lca.jrc.it/ILCD/Contact\" xmlns:common=\"http://lca.jrc.it/ILCD/Common\" xmlns:epd=\"http://www.iai.kit.edu/EPD/2013\" xmlns:epd2=\"http://www.indata.network/EPD/2019\" xmlns:f=\"http://lca.jrc.it/ILCD/Flow\" xmlns:fp=\"http://lca.jrc.it/ILCD/FlowProperty\" xmlns:m=\"http://lca.jrc.it/ILCD/LCIAMethod\" xmlns:s=\"http://lca.jrc.it/ILCD/Source\" xmlns:u=\"http://lca.jrc.it/ILCD/UnitGroup\" name=\"B1\" scenario=\"Standard Scenario\"/>", "<ns11:modules xmlns:ns11=\"http://openlca.org/epd_ilcd\" xmlns=\"http://lca.jrc.it/ILCD/Process\" xmlns:c=\"http://lca.jrc.it/ILCD/Contact\" xmlns:common=\"http://lca.jrc.it/ILCD/Common\" xmlns:epd=\"http://www.iai.kit.edu/EPD/2013\" xmlns:epd2=\"http://www.indata.network/EPD/2019\" xmlns:f=\"http://lca.jrc.it/ILCD/Flow\" xmlns:fp=\"http://lca.jrc.it/ILCD/FlowProperty\" xmlns:m=\"http://lca.jrc.it/ILCD/LCIAMethod\" xmlns:s=\"http://lca.jrc.it/ILCD/Source\" xmlns:u=\"http://lca.jrc.it/ILCD/UnitGroup\" name=\"B2\" scenario=\"Standard Scenario\"/>", "<ns11:modules xmlns:ns11=\"http://openlca.org/epd_ilcd\" xmlns=\"http://lca.jrc.it/ILCD/Process\" xmlns:c=\"http://lca.jrc.it/ILCD/Contact\" xmlns:common=\"http://lca.jrc.it/ILCD/Common\" xmlns:epd=\"http://www.iai.kit.edu/EPD/2013\" xmlns:epd2=\"http://www.indata.network/EPD/2019\" xmlns:f=\"http://lca.jrc.it/ILCD/Flow\" xmlns:fp=\"http://lca.jrc.it/ILCD/FlowProperty\" xmlns:m=\"http://lca.jrc.it/ILCD/LCIAMethod\" xmlns:s=\"http://lca.jrc.it/ILCD/Source\" xmlns:u=\"http://lca.jrc.it/ILCD/UnitGroup\" name=\"B3\" scenario=\"Standard Scenario\"/>", "<ns11:modules xmlns:ns11=\"http://openlca.org/epd_ilcd\" xmlns=\"http://lca.jrc.it/ILCD/Process\" xmlns:c=\"http://lca.jrc.it/ILCD/Contact\" xmlns:common=\"http://lca.jrc.it/ILCD/Common\" xmlns:epd=\"http://www.iai.kit.edu/EPD/2013\" xmlns:epd2=\"http://www.indata.network/EPD/2019\" xmlns:f=\"http://lca.jrc.it/ILCD/Flow\" xmlns:fp=\"http://lca.jrc.it/ILCD/FlowProperty\" xmlns:m=\"http://lca.jrc.it/ILCD/LCIAMethod\" xmlns:s=\"http://lca.jrc.it/ILCD/Source\" xmlns:u=\"http://lca.jrc.it/ILCD/UnitGroup\" name=\"B6\" scenario=\"Standard Scenario\"/>", "<ns11:modules xmlns:ns11=\"http://openlca.org/epd_ilcd\" xmlns=\"http://lca.jrc.it/ILCD/Process\" xmlns:c=\"http://lca.jrc.it/ILCD/Contact\" xmlns:common=\"http://lca.jrc.it/ILCD/Common\" xmlns:epd=\"http://www.iai.kit.edu/EPD/2013\" xmlns:epd2=\"http://www.indata.network/EPD/2019\" xmlns:f=\"http://lca.jrc.it/ILCD/Flow\" xmlns:fp=\"http://lca.jrc.it/ILCD/FlowProperty\" xmlns:m=\"http://lca.jrc.it/ILCD/LCIAMethod\" xmlns:s=\"http://lca.jrc.it/ILCD/Source\" xmlns:u=\"http://lca.jrc.it/ILCD/UnitGroup\" name=\"B7\" scenario=\"Standard Scenario\"/>", "<ns11:modules xmlns:ns11=\"http://openlca.org/epd_ilcd\" xmlns=\"http://lca.jrc.it/ILCD/Process\" xmlns:c=\"http://lca.jrc.it/ILCD/Contact\" xmlns:common=\"http://lca.jrc.it/ILCD/Common\" xmlns:epd=\"http://www.iai.kit.edu/EPD/2013\" xmlns:epd2=\"http://www.indata.network/EPD/2019\" xmlns:f=\"http://lca.jrc.it/ILCD/Flow\" xmlns:fp=\"http://lca.jrc.it/ILCD/FlowProperty\" xmlns:m=\"http://lca.jrc.it/ILCD/LCIAMethod\" xmlns:s=\"http://lca.jrc.it/ILCD/Source\" xmlns:u=\"http://lca.jrc.it/ILCD/UnitGroup\" name=\"C1\" scenario=\"Standard Scenario\"/>", "<ns11:modules xmlns:ns11=\"http://openlca.org/epd_ilcd\" xmlns=\"http://lca.jrc.it/ILCD/Process\" xmlns:c=\"http://lca.jrc.it/ILCD/Contact\" xmlns:common=\"http://lca.jrc.it/ILCD/Common\" xmlns:epd=\"http://www.iai.kit.edu/EPD/2013\" xmlns:epd2=\"http://www.indata.network/EPD/2019\" xmlns:f=\"http://lca.jrc.it/ILCD/Flow\" xmlns:fp=\"http://lca.jrc.it/ILCD/FlowProperty\" xmlns:m=\"http://lca.jrc.it/ILCD/LCIAMethod\" xmlns:s=\"http://lca.jrc.it/ILCD/Source\" xmlns:u=\"http://lca.jrc.it/ILCD/UnitGroup\" name=\"C2\" scenario=\"Standard Scenario\"/>", "<ns11:modules xmlns:ns11=\"http://openlca.org/epd_ilcd\" xmlns=\"http://lca.jrc.it/ILCD/Process\" xmlns:c=\"http://lca.jrc.it/ILCD/Contact\" xmlns:common=\"http://lca.jrc.it/ILCD/Common\" xmlns:epd=\"http://www.iai.kit.edu/EPD/2013\" xmlns:epd2=\"http://www.indata.network/EPD/2019\" xmlns:f=\"http://lca.jrc.it/ILCD/Flow\" xmlns:fp=\"http://lca.jrc.it/ILCD/FlowProperty\" xmlns:m=\"http://lca.jrc.it/ILCD/LCIAMethod\" xmlns:s=\"http://lca.jrc.it/ILCD/Source\" xmlns:u=\"http://lca.jrc.it/ILCD/UnitGroup\" name=\"C3\" scenario=\"Standard Scenario\"/>", "<ns11:modules xmlns:ns11=\"http://openlca.org/epd_ilcd\" xmlns=\"http://lca.jrc.it/ILCD/Process\" xmlns:c=\"http://lca.jrc.it/ILCD/Contact\" xmlns:common=\"http://lca.jrc.it/ILCD/Common\" xmlns:epd=\"http://www.iai.kit.edu/EPD/2013\" xmlns:epd2=\"http://www.indata.network/EPD/2019\" xmlns:f=\"http://lca.jrc.it/ILCD/Flow\" xmlns:fp=\"http://lca.jrc.it/ILCD/FlowProperty\" xmlns:m=\"http://lca.jrc.it/ILCD/LCIAMethod\" xmlns:s=\"http://lca.jrc.it/ILCD/Source\" xmlns:u=\"http://lca.jrc.it/ILCD/UnitGroup\" name=\"C4\" scenario=\"Standard Scenario\"/>", "<ns11:modules xmlns:ns11=\"http://openlca.org/epd_ilcd\" xmlns=\"http://lca.jrc.it/ILCD/Process\" xmlns:c=\"http://lca.jrc.it/ILCD/Contact\" xmlns:common=\"http://lca.jrc.it/ILCD/Common\" xmlns:epd=\"http://www.iai.kit.edu/EPD/2013\" xmlns:epd2=\"http://www.indata.network/EPD/2019\" xmlns:f=\"http://lca.jrc.it/ILCD/Flow\" xmlns:fp=\"http://lca.jrc.it/ILCD/FlowProperty\" xmlns:m=\"http://lca.jrc.it/ILCD/LCIAMethod\" xmlns:s=\"http://lca.jrc.it/ILCD/Source\" xmlns:u=\"http://lca.jrc.it/ILCD/UnitGroup\" name=\"D\" scenario=\"Standard Scenario\"/>"]}}, "quantitativeReference": {"referenceToReferenceFlow": [1], "type": "Reference flow(s)"}, "time": {"referenceYear": 2023, "dataSetValidUntil": 2030, "timeRepresentativenessDescription": [{"value": "Data gathering: From 7th of September 2023 till 26th of September 2024. Reference period: 2023", "lang": "en"}], "other": {"anies": [{"name": "publicationDateOfEPD", "value": 1740528000000}]}}, "geography": {"locationOfOperationSupplyOrProduction": {"descriptionOfRestrictions": [{"value": "The results of this EPD are representative for European Union. \r", "lang": "en"}], "location": "EU-27"}}, "technology": {"technologyDescriptionAndIncludedProcesses": [{"value": "Radon Barrier Protection Systems have been developed to provide a flexible solution for radon protection (and protection against moisture) in dwellings, schools and other buildings. Radon membranes are manufactured by a polythene extrusion process. 3 to 4 machines are involved for each product being 1. blown film: a process that involves melting plastic pellets and extruding them through a circular die. As the plastic is extruded, the air is blown into the center of the die, causing the molten plastic to expand into a bubble or tube 2. coater: The coater process involving melting plastic pellets is typically part of a hot melt coating or extrusion coating system. This process is widely used in industries such as packaging. 3. grid (optional, when there is a reinforcement): In this process, polyester yarns are knitted into a net using warp knitting machines. The machines glue the threads together with wax 4. rewinder: A film rewinder is a device used to rewind film from one large roll (so called jumbo roll) into smaller rolls or to adjust the tension, width and quality of the film.", "lang": "en"}], "technologicalApplicability": [{"value": "They are used to protect buildings from the ingress of radon gas. It is a loose-laid membrane and may be installed below or above a ground-bearing slab, or on top of a suspended concrete floor. ", "lang": "en"}], "referenceToTechnologyFlowDiagrammOrPicture": [{"shortDescription": [{"value": "Flow Chart for Monarflex Necoseal (BMI Group Holdings UK Limited)", "lang": "en"}], "type": "source data set", "refObjectId": "1531fde8-66e0-4827-b1ee-61c7ab3e8f71", "version": "00.00.001"}]}}, "modellingAndValidation": {"LCIMethodAndAllocation": {"typeOfDataSet": "EPD", "other": {"anies": [{"name": "subType", "value": "specific dataset"}]}}, "dataSourcesTreatmentAndRepresentativeness": {"referenceToDataSource": [{"shortDescription": [{"value": "ecoinvent database (general)", "lang": "en"}], "type": "source data set", "refObjectId": "b497a91f-e14b-4b69-8f28-f50eb1576766", "version": "00.03.002"}, {"shortDescription": [{"value": "ecoinvent 3.6 database", "lang": "en"}], "type": "source data set", "refObjectId": "766b9973-5ee8-48a2-8098-72c8e20b369f", "version": "00.00.001"}], "useAdviceForDataSet": [{"value": "They are used to protect buildings from the ingress of radon gas. It is a loose-laid membrane and may be installed below or above a ground-bearing slab, or on top of a suspended concrete floor. ", "lang": "en"}], "other": {"anies": [{"name": "referenceToOriginalEPD", "value": {"shortDescription": {"value": "EPD for Monarflex Necoseal (BMI Group Holdings UK Limited)", "defaultValue": "EPD for Monarflex Necoseal (BMI Group Holdings UK Limited)", "lstrings": [{"lang": "en", "value": "EPD for Monarflex Necoseal (BMI Group Holdings UK Limited)"}]}, "version": {"version": 1, "majorVersion": 0, "minorVersion": 0, "subMinorVersion": 1, "zero": false, "versionString": "00.00.001"}, "type": "source data set", "uuid": {"uuid": "fff0d5ba-4014-46af-b10e-dd27da86ab39"}, "refObjectId": "fff0d5ba-4014-46af-b10e-dd27da86ab39", "versionAsString": "00.00.001", "resourceURLs": ["https://oekobaudat.de/OEKOBAU.DAT/resource/sources/fff0d5ba-4014-46af-b10e-dd27da86ab39/EPD-Kiwa-EE-192464-EN.pdf?version=00.00.001"]}}]}}, "validation": {"review": [{"reviewDetails": [{"value": "The independent verification is in accordance with the ISO 14025:2011.", "lang": "en"}], "referenceToNameOfReviewerAndInstitution": [{"shortDescription": [{"value": "Anne Kees Jeeninga, Advieslab", "lang": "en"}], "type": "contact data set", "refObjectId": "f40584c8-fc89-48d3-a501-42cb5007cb13", "version": "00.00.001"}], "type": "Independent external review"}]}, "complianceDeclarations": {"compliance": [{"referenceToComplianceSystem": {"shortDescription": [{"value": "EN 15804+A2 (EF 3.0)", "lang": "de"}, {"value": "EN 15804+A2 (EF 3.0)", "lang": "en"}], "type": "source data set", "refObjectId": "c0016b33-8cf7-415c-ac6e-deba0d21440d", "version": "00.02.000"}}, {"referenceToComplianceSystem": {"shortDescription": [{"value": "ISO 14025", "lang": "en"}], "type": "source data set", "refObjectId": "4f2eb655-6e44-4874-a95a-e28f5442cd4d", "version": "00.00.001"}}]}}, "administrativeInformation": {"commissionerAndGoal": {"referenceToCommissioner": [{"shortDescription": [{"value": "BMI Group Holdings UK Limited", "lang": "en"}], "type": "contact data set", "refObjectId": "779569e3-92d4-4970-8cbe-7b27addb2782", "version": "00.00.001"}]}, "dataGenerator": {"referenceToPersonOrEntityGeneratingTheDataSet": [{"shortDescription": [{"value": "BMI Group Holdings UK Limited", "lang": "en"}], "type": "contact data set", "refObjectId": "779569e3-92d4-4970-8cbe-7b27addb2782", "version": "00.00.001"}]}, "dataEntryBy": {"timeStamp": 1750774000266, "referenceToDataSetFormat": [{"shortDescription": [{"value": "ILCD format", "lang": "en"}], "type": "source data set", "refObjectId": "a97a0155-0234-4b87-b4ce-a45da52f2a40", "version": "01.00.000", "uri": "http://lca.jrc.ec.europa.eu/lcainfohub/sample_data/ilcd/sources/ILCD_Format_a97a0155-0234-4b87-b4ce-a45da52f2a40_01.00.000.xml"}, {"shortDescription": [{"value": "EPD Data Format Extensions v1.2", "lang": "en"}, {"value": "EPD-Datenformaterweiterungen v1.2", "lang": "de"}], "type": "source data set", "refObjectId": "a29449fd-aa2f-4de8-b5d7-4b06b43c6fde", "version": "00.01.000"}], "referenceToPersonOrEntityEnteringTheData": {"shortDescription": [{"value": "Kiwa GmbH (Berlin)", "lang": "en"}], "type": "contact data set", "refObjectId": "3ea4a87a-3f88-4633-b7e7-1bbdd272be43", "version": "00.00.002"}}, "publicationAndOwnership": {"dataSetVersion": "00.00.013", "referenceToRegistrationAuthority": {"shortDescription": [{"value": "Kiwa-Ecobility Experts, Kiwa GmbH (Berlin)", "lang": "en"}], "type": "contact data set", "refObjectId": "eb52a9a8-9d0f-40ce-a5c9-7b78f5615e5a", "version": "00.00.002"}, "registrationNumber": "EPD-Kiwa-EE-192464-EN", "referenceToOwnershipOfDataSet": {"shortDescription": [{"value": "BMI Group Holdings UK Limited", "lang": "en"}], "type": "contact data set", "refObjectId": "779569e3-92d4-4970-8cbe-7b27addb2782", "version": "00.00.001"}, "copyright": true, "licenseType": "Free of charge for all users and uses", "accessRestrictions": [{"value": "None", "lang": "en"}], "other": {"anies": [{"name": "referenceToPublisher", "value": {"shortDescription": [{"value": "Kiwa-Ecobility Experts, Kiwa GmbH (Berlin)", "lang": "en"}], "type": "contact data set", "refObjectId": "eb52a9a8-9d0f-40ce-a5c9-7b78f5615e5a", "version": "00.00.002"}}]}}}, "exchanges": {"exchange": [{"dataSetInternalID": 1, "referenceToFlowDataSet": {"shortDescription": [{"value": "Monarflex Necoseal (BMI Group Holdings UK Limited)", "lang": "en"}], "type": "flow data set", "refObjectId": "f97db581-1b9f-404c-addc-df43973073c1", "version": "00.00.001"}, "meanAmount": 1.0, "resultingAmount": 1.0, "referenceFlow": true, "resultingflowAmount": 1.0, "flowProperties": [{"name": [{"lang": "de", "value": "Fläche"}, {"lang": "en", "value": "Area"}], "uuid": "93a60a56-a3c8-19da-a746-0800200c9a66", "referenceFlowProperty": true, "meanValue": 1.0, "referenceUnit": "qm", "unitGroupUUID": "c20a03d7-bd90-4569-bc94-66cfd364dfc8"}], "materialProperties": [{"name": "layer thickness", "value": "3.4E-4", "unit": "m", "unitDescription": "meters"}, {"name": "grammage", "value": "0.309", "unit": "kg/m^2", "unitDescription": "kilograms per square meter"}], "typeOfFlow": "Product flow", "classification": {"classHierarchy": "Kunststoffe / Folien und Vliese / Unterspannbahn", "name": "OEKOBAU.DAT"}}, {"dataSetInternalID": 2, "referenceToFlowDataSet": {"shortDescription": [{"value": "Components for re-use (CRU)", "lang": "en"}, {"value": "Komponenten für die Wiederverwendung (CRU)", "lang": "de"}, {"value": "Componentes para su reutilización (CRU)", "lang": "es"}], "type": "flow data set", "refObjectId": "a2b32f97-3fc7-4af2-b209-525bc6426f33", "version": "30.00.000", "uri": "../flows/a2b32f97-3fc7-4af2-b209-525bc6426f33.xml"}, "exchange direction": "OUTPUT", "meanAmount": 0.0, "other": {"anies": [{"value": "0.0", "module": "A1", "scenario": "Standard Scenario"}, {"value": "0.0", "module": "A2", "scenario": "Standard Scenario"}, {"value": "0.0", "module": "A3", "scenario": "Standard Scenario"}, {"value": "0.0", "module": "A1-A3", "scenario": "Standard Scenario"}, {"value": "0.0", "module": "A4", "scenario": "Standard Scenario"}, {"value": "0.0", "module": "A5", "scenario": "Standard Scenario"}, {"value": "0.0", "module": "B1", "scenario": "Standard Scenario"}, {"value": "0.0", "module": "B2", "scenario": "Standard Scenario"}, {"value": "0.0", "module": "B3", "scenario": "Standard Scenario"}, {"value": "0.0", "module": "B6", "scenario": "Standard Scenario"}, {"value": "0.0", "module": "B7", "scenario": "Standard Scenario"}, {"value": "0.0", "module": "C1", "scenario": "Standard Scenario"}, {"value": "0.0", "module": "C2", "scenario": "Standard Scenario"}, {"value": "0.0", "module": "C3", "scenario": "Standard Scenario"}, {"value": "0.0", "module": "C4", "scenario": "Standard Scenario"}, {"value": "0.0", "module": "D", "scenario": "Standard Scenario"}, {"name": "referenceToUnitGroupDataSet", "value": {"shortDescription": [{"value": "kg", "lang": "en"}], "type": "unit group data set", "refObjectId": "ad38d542-3fe9-439d-9b95-2f5f7752acaf", "version": "30.00.000", "uri": "../unitgroups/ad38d542-3fe9-439d-9b95-2f5f7752acaf.xml"}}]}, "flowProperties": [], "typeOfFlow": "Other flow", "classification": {"classHierarchy": "Größen / Umweltliche Größen / EPD EN 15804 / LCI Indikatoren", "name": "GaBiCategories"}}, {"dataSetInternalID": 3, "referenceToFlowDataSet": {"shortDescription": [{"value": "Exported electrical energy (EEE)", "lang": "en"}, {"value": "Exportierte elektrische Energie (EEE)", "lang": "de"}, {"value": "Energía exportada electrica (EEE)", "lang": "es"}], "type": "flow data set", "refObjectId": "4da0c987-2b76-40d6-9e9e-82a017aaaf29", "version": "30.00.000", "uri": "../flows/4da0c987-2b76-40d6-9e9e-82a017aaaf29.xml"}, "exchange direction": "OUTPUT", "meanAmount": 0.0, "other": {"anies": [{"value": "0.0", "module": "A1", "scenario": "Standard Scenario"}, {"value": "0.0", "module": "A2", "scenario": "Standard Scenario"}, {"value": "0.0", "module": "A3", "scenario": "Standard Scenario"}, {"value": "0.0", "module": "A1-A3", "scenario": "Standard Scenario"}, {"value": "0.0", "module": "A4", "scenario": "Standard Scenario"}, {"value": "0.0", "module": "A5", "scenario": "Standard Scenario"}, {"value": "0.0", "module": "B1", "scenario": "Standard Scenario"}, {"value": "0.0", "module": "B2", "scenario": "Standard Scenario"}, {"value": "0.0", "module": "B3", "scenario": "Standard Scenario"}, {"value": "0.0", "module": "B6", "scenario": "Standard Scenario"}, {"value": "0.0", "module": "B7", "scenario": "Standard Scenario"}, {"value": "0.0", "module": "C1", "scenario": "Standard Scenario"}, {"value": "0.0", "module": "C2", "scenario": "Standard Scenario"}, {"value": "0.0", "module": "C3", "scenario": "Standard Scenario"}, {"value": "0.0", "module": "C4", "scenario": "Standard Scenario"}, {"value": "-2.07324442219683", "module": "D", "scenario": "Standard Scenario"}, {"name": "referenceToUnitGroupDataSet", "value": {"shortDescription": [{"value": "MJ", "lang": "en"}], "type": "unit group data set", "refObjectId": "93a60a57-a3c8-11da-a746-0800200c9a66", "version": "03.00.000", "uri": "../unitgroups/93a60a57-a3c8-11da-a746-0800200c9a66.xml"}}]}, "flowProperties": [], "typeOfFlow": "Other flow", "classification": {"classHierarchy": "Größen / Umweltliche Größen / EPD EN 15804 / LCI Indikatoren", "name": "GaBiCategories"}}, {"dataSetInternalID": 4, "referenceToFlowDataSet": {"shortDescription": [{"value": "Exported thermal energy (EET)", "lang": "en"}, {"value": "Exportierte thermische Energie (EET)", "lang": "de"}, {"value": "Energía exportada termal (EET)", "lang": "es"}], "type": "flow data set", "refObjectId": "98daf38a-7a79-46d3-9a37-2b7bd0955810", "version": "30.00.000", "uri": "../flows/98daf38a-7a79-46d3-9a37-2b7bd0955810.xml"}, "exchange direction": "OUTPUT", "meanAmount": 0.0, "other": {"anies": [{"value": "0.0", "module": "A1", "scenario": "Standard Scenario"}, {"value": "0.0", "module": "A2", "scenario": "Standard Scenario"}, {"value": "0.0", "module": "A3", "scenario": "Standard Scenario"}, {"value": "0.0", "module": "A1-A3", "scenario": "Standard Scenario"}, {"value": "0.0", "module": "A4", "scenario": "Standard Scenario"}, {"value": "0.0", "module": "A5", "scenario": "Standard Scenario"}, {"value": "0.0", "module": "B1", "scenario": "Standard Scenario"}, {"value": "0.0", "module": "B2", "scenario": "Standard Scenario"}, {"value": "0.0", "module": "B3", "scenario": "Standard Scenario"}, {"value": "0.0", "module": "B6", "scenario": "Standard Scenario"}, {"value": "0.0", "module": "B7", "scenario": "Standard Scenario"}, {"value": "0.0", "module": "C1", "scenario": "Standard Scenario"}, {"value": "0.0", "module": "C2", "scenario": "Standard Scenario"}, {"value": "0.0", "module": "C3", "scenario": "Standard Scenario"}, {"value": "0.0", "module": "C4", "scenario": "Standard Scenario"}, {"value": "-3.57058761600565", "module": "D", "scenario": "Standard Scenario"}, {"name": "referenceToUnitGroupDataSet", "value": {"shortDescription": [{"value": "MJ", "lang": "en"}], "type": "unit group data set", "refObjectId": "93a60a57-a3c8-11da-a746-0800200c9a66", "version": "03.00.000", "uri": "../unitgroups/93a60a57-a3c8-11da-a746-0800200c9a66.xml"}}]}, "flowProperties": [], "typeOfFlow": "Other flow", "classification": {"classHierarchy": "Größen / Umweltliche Größen / EPD EN 15804 / LCI Indikatoren", "name": "GaBiCategories"}}, {"dataSetInternalID": 5, "referenceToFlowDataSet": {"shortDescription": [{"value": "Use of net fresh water (FW)", "lang": "en"}, {"value": "Einsatz von Süßwasserressourcen (FW)", "lang": "de"}, {"value": "Uso neto de recursos de agua dulce (FW)", "lang": "es"}], "type": "flow data set", "refObjectId": "3cf952c8-f3a4-461d-8c96-96456ca62246", "version": "30.00.000", "uri": "../flows/3cf952c8-f3a4-461d-8c96-96456ca62246.xml"}, "exchange direction": "INPUT", "meanAmount": 0.0, "other": {"anies": [{"value": "0.01074489797315", "module": "A1", "scenario": "Standard Scenario"}, {"value": "2.720284576E-5", "module": "A2", "scenario": "Standard Scenario"}, {"value": "0.00212251997571", "module": "A3", "scenario": "Standard Scenario"}, {"value": "0.01289462079462", "module": "A1-A3", "scenario": "Standard Scenario"}, {"value": "9.627669749E-5", "module": "A4", "scenario": "Standard Scenario"}, {"value": "7.2000805257E-4", "module": "A5", "scenario": "Standard Scenario"}, {"value": "0.0", "module": "B1", "scenario": "Standard Scenario"}, {"value": "0.0", "module": "B2", "scenario": "Standard Scenario"}, {"value": "0.0", "module": "B3", "scenario": "Standard Scenario"}, {"value": "0.0", "module": "B6", "scenario": "Standard Scenario"}, {"value": "0.0", "module": "B7", "scenario": "Standard Scenario"}, {"value": "0.0", "module": "C1", "scenario": "Standard Scenario"}, {"value": "1.06740747E-5", "module": "C2", "scenario": "Standard Scenario"}, {"value": "0.00104490024867", "module": "C3", "scenario": "Standard Scenario"}, {"value": "8.05697324E-6", "module": "C4", "scenario": "Standard Scenario"}, {"value": "-7.2043041303E-4", "module": "D", "scenario": "Standard Scenario"}, {"name": "referenceToUnitGroupDataSet", "value": {"shortDescription": [{"value": "m3", "lang": "en"}], "type": "unit group data set", "refObjectId": "cd950537-0a98-4044-9ba7-9f9a68d0a504", "version": "30.00.000", "uri": "../unitgroups/cd950537-0a98-4044-9ba7-9f9a68d0a504.xml"}}]}, "flowProperties": [], "typeOfFlow": "Other flow", "classification": {"classHierarchy": "Größen / Umweltliche Größen / EPD EN 15804 / LCI Indikatoren", "name": "GaBiCategories"}}, {"dataSetInternalID": 6, "referenceToFlowDataSet": {"shortDescription": [{"value": "Hazardous waste disposed (HWD)", "lang": "en"}, {"value": "Gefährlicher Abfall zur Deponie (HWD)", "lang": "de"}, {"value": "Residuos peligrosos eliminados (HWD)", "lang": "es"}], "type": "flow data set", "refObjectId": "430f9e0f-59b2-46a0-8e0d-55e0e84948fc", "version": "30.00.000", "uri": "../flows/430f9e0f-59b2-46a0-8e0d-55e0e84948fc.xml"}, "exchange direction": "OUTPUT", "meanAmount": 0.0, "other": {"anies": [{"value": "2.95221E-6", "module": "A1", "scenario": "Standard Scenario"}, {"value": "5.6590942E-7", "module": "A2", "scenario": "Standard Scenario"}, {"value": "2.43776542E-6", "module": "A3", "scenario": "Standard Scenario"}, {"value": "5.95588484E-6", "module": "A1-A3", "scenario": "Standard Scenario"}, {"value": "2.00287465E-6", "module": "A4", "scenario": "Standard Scenario"}, {"value": "5.4189117E-7", "module": "A5", "scenario": "Standard Scenario"}, {"value": "0.0", "module": "B1", "scenario": "Standard Scenario"}, {"value": "0.0", "module": "B2", "scenario": "Standard Scenario"}, {"value": "0.0", "module": "B3", "scenario": "Standard Scenario"}, {"value": "0.0", "module": "B6", "scenario": "Standard Scenario"}, {"value": "0.0", "module": "B7", "scenario": "Standard Scenario"}, {"value": "0.0", "module": "C1", "scenario": "Standard Scenario"}, {"value": "2.2205616E-7", "module": "C2", "scenario": "Standard Scenario"}, {"value": "1.02142124E-6", "module": "C3", "scenario": "Standard Scenario"}, {"value": "1.171644E-8", "module": "C4", "scenario": "Standard Scenario"}, {"value": "-1.009462812E-5", "module": "D", "scenario": "Standard Scenario"}, {"name": "referenceToUnitGroupDataSet", "value": {"shortDescription": [{"value": "kg", "lang": "en"}], "type": "unit group data set", "refObjectId": "ad38d542-3fe9-439d-9b95-2f5f7752acaf", "version": "30.00.000", "uri": "../unitgroups/ad38d542-3fe9-439d-9b95-2f5f7752acaf.xml"}}]}, "flowProperties": [], "typeOfFlow": "Other flow", "classification": {"classHierarchy": "Größen / Umweltliche Größen / EPD EN 15804 / LCI Indikatoren", "name": "GaBiCategories"}}, {"dataSetInternalID": 7, "referenceToFlowDataSet": {"shortDescription": [{"value": "Materials for energy recovery (MER)", "lang": "en"}, {"value": "Stoffe für die Energierückgewinnung (MER)", "lang": "de"}, {"value": "Materiales para valorización energética (recuperación de energía) (MER)", "lang": "es"}], "type": "flow data set", "refObjectId": "59a9181c-3aaf-46ee-8b13-2b3723b6e447", "version": "30.00.000", "uri": "../flows/59a9181c-3aaf-46ee-8b13-2b3723b6e447.xml"}, "exchange direction": "OUTPUT", "meanAmount": 0.0, "other": {"anies": [{"value": "0.0", "module": "A1", "scenario": "Standard Scenario"}, {"value": "0.0", "module": "A2", "scenario": "Standard Scenario"}, {"value": "0.0", "module": "A3", "scenario": "Standard Scenario"}, {"value": "0.0", "module": "A1-A3", "scenario": "Standard Scenario"}, {"value": "0.0", "module": "A4", "scenario": "Standard Scenario"}, {"value": "0.0", "module": "A5", "scenario": "Standard Scenario"}, {"value": "0.0", "module": "B1", "scenario": "Standard Scenario"}, {"value": "0.0", "module": "B2", "scenario": "Standard Scenario"}, {"value": "0.0", "module": "B3", "scenario": "Standard Scenario"}, {"value": "0.0", "module": "B6", "scenario": "Standard Scenario"}, {"value": "0.0", "module": "B7", "scenario": "Standard Scenario"}, {"value": "0.0", "module": "C1", "scenario": "Standard Scenario"}, {"value": "0.0", "module": "C2", "scenario": "Standard Scenario"}, {"value": "0.0", "module": "C3", "scenario": "Standard Scenario"}, {"value": "0.0", "module": "C4", "scenario": "Standard Scenario"}, {"value": "0.0", "module": "D", "scenario": "Standard Scenario"}, {"name": "referenceToUnitGroupDataSet", "value": {"shortDescription": [{"value": "kg", "lang": "en"}], "type": "unit group data set", "refObjectId": "ad38d542-3fe9-439d-9b95-2f5f7752acaf", "version": "30.00.000", "uri": "../unitgroups/ad38d542-3fe9-439d-9b95-2f5f7752acaf.xml"}}]}, "flowProperties": [], "typeOfFlow": "Other flow", "classification": {"classHierarchy": "Größen / Umweltliche Größen / EPD EN 15804 / LCI Indikatoren", "name": "GaBiCategories"}}, {"dataSetInternalID": 8, "referenceToFlowDataSet": {"shortDescription": [{"value": "Materials for recycling (MFR)", "lang": "en"}, {"value": "Stoffe zum Recycling (MFR)", "lang": "de"}, {"value": "Materiales para el reciclaje (MFR)", "lang": "es"}], "type": "flow data set", "refObjectId": "d7fe48a5-4103-49c8-9aae-b0b5dfdbd6ae", "version": "30.00.000", "uri": "../flows/d7fe48a5-4103-49c8-9aae-b0b5dfdbd6ae.xml"}, "exchange direction": "OUTPUT", "meanAmount": 0.0, "other": {"anies": [{"value": "0.0", "module": "A1", "scenario": "Standard Scenario"}, {"value": "0.0", "module": "A2", "scenario": "Standard Scenario"}, {"value": "0.0", "module": "A3", "scenario": "Standard Scenario"}, {"value": "0.0", "module": "A1-A3", "scenario": "Standard Scenario"}, {"value": "0.0", "module": "A4", "scenario": "Standard Scenario"}, {"value": "0.02888254515625", "module": "A5", "scenario": "Standard Scenario"}, {"value": "0.0", "module": "B1", "scenario": "Standard Scenario"}, {"value": "0.0", "module": "B2", "scenario": "Standard Scenario"}, {"value": "0.0", "module": "B3", "scenario": "Standard Scenario"}, {"value": "0.0", "module": "B6", "scenario": "Standard Scenario"}, {"value": "0.0", "module": "B7", "scenario": "Standard Scenario"}, {"value": "0.0", "module": "C1", "scenario": "Standard Scenario"}, {"value": "0.0", "module": "C2", "scenario": "Standard Scenario"}, {"value": "0.015375903125", "module": "C3", "scenario": "Standard Scenario"}, {"value": "0.0", "module": "C4", "scenario": "Standard Scenario"}, {"value": "0.0", "module": "D", "scenario": "Standard Scenario"}, {"name": "referenceToUnitGroupDataSet", "value": {"shortDescription": [{"value": "kg", "lang": "en"}], "type": "unit group data set", "refObjectId": "ad38d542-3fe9-439d-9b95-2f5f7752acaf", "version": "30.00.000", "uri": "../unitgroups/ad38d542-3fe9-439d-9b95-2f5f7752acaf.xml"}}]}, "flowProperties": [], "typeOfFlow": "Other flow", "classification": {"classHierarchy": "Größen / Umweltliche Größen / EPD EN 15804 / LCI Indikatoren", "name": "GaBiCategories"}}, {"dataSetInternalID": 9, "referenceToFlowDataSet": {"shortDescription": [{"value": "Non-hazardous waste disposed (NHWD)", "lang": "en"}, {"value": "Entsorgter nicht gefährlicher Abfall (NHWD)", "lang": "de"}, {"value": "Residuos no peligrosos eliminados (NHWD)", "lang": "es"}], "type": "flow data set", "refObjectId": "b29ef66b-e286-4afa-949f-62f1a7b4d7fa", "version": "30.00.000", "uri": "../flows/b29ef66b-e286-4afa-949f-62f1a7b4d7fa.xml"}, "exchange direction": "OUTPUT", "meanAmount": 0.0, "other": {"anies": [{"value": "0.0258162764657", "module": "A1", "scenario": "Standard Scenario"}, {"value": "0.01416584369254", "module": "A2", "scenario": "Standard Scenario"}, {"value": "0.00887512430082", "module": "A3", "scenario": "Standard Scenario"}, {"value": "0.04885724445906", "module": "A1-A3", "scenario": "Standard Scenario"}, {"value": "0.0501359548915", "module": "A4", "scenario": "Standard Scenario"}, {"value": "0.0096560823041", "module": "A5", "scenario": "Standard Scenario"}, {"value": "0.0", "module": "B1", "scenario": "Standard Scenario"}, {"value": "0.0", "module": "B2", "scenario": "Standard Scenario"}, {"value": "0.0", "module": "B3", "scenario": "Standard Scenario"}, {"value": "0.0", "module": "B6", "scenario": "Standard Scenario"}, {"value": "0.0", "module": "B7", "scenario": "Standard Scenario"}, {"value": "0.0", "module": "C1", "scenario": "Standard Scenario"}, {"value": "0.00555850939671", "module": "C2", "scenario": "Standard Scenario"}, {"value": "0.01289435536785", "module": "C3", "scenario": "Standard Scenario"}, {"value": "0.03082613336571", "module": "C4", "scenario": "Standard Scenario"}, {"value": "-0.00467994021465", "module": "D", "scenario": "Standard Scenario"}, {"name": "referenceToUnitGroupDataSet", "value": {"shortDescription": [{"value": "kg", "lang": "en"}], "type": "unit group data set", "refObjectId": "ad38d542-3fe9-439d-9b95-2f5f7752acaf", "version": "30.00.000", "uri": "../unitgroups/ad38d542-3fe9-439d-9b95-2f5f7752acaf.xml"}}]}, "flowProperties": [], "typeOfFlow": "Other flow", "classification": {"classHierarchy": "Größen / Umweltliche Größen / EPD EN 15804 / LCI Indikatoren", "name": "GaBiCategories"}}, {"dataSetInternalID": 10, "referenceToFlowDataSet": {"shortDescription": [{"value": "Use of non renewable secondary fuels (NRSF)", "lang": "en"}, {"value": "Nicht erneuerbare Sekundärbrennstoffe (NRSF)", "lang": "de"}, {"value": "Uso de combustibles secundarios no renovables (NRSF)", "lang": "es"}], "type": "flow data set", "refObjectId": "89def144-d39a-4287-b86f-efde453ddcb2", "version": "30.00.000", "uri": "../flows/89def144-d39a-4287-b86f-efde453ddcb2.xml"}, "exchange direction": "INPUT", "meanAmount": 0.0, "other": {"anies": [{"value": "0.0", "module": "A1", "scenario": "Standard Scenario"}, {"value": "0.0", "module": "A2", "scenario": "Standard Scenario"}, {"value": "0.0", "module": "A3", "scenario": "Standard Scenario"}, {"value": "0.0", "module": "A1-A3", "scenario": "Standard Scenario"}, {"value": "0.0", "module": "A4", "scenario": "Standard Scenario"}, {"value": "0.0", "module": "A5", "scenario": "Standard Scenario"}, {"value": "0.0", "module": "B1", "scenario": "Standard Scenario"}, {"value": "0.0", "module": "B2", "scenario": "Standard Scenario"}, {"value": "0.0", "module": "B3", "scenario": "Standard Scenario"}, {"value": "0.0", "module": "B6", "scenario": "Standard Scenario"}, {"value": "0.0", "module": "B7", "scenario": "Standard Scenario"}, {"value": "0.0", "module": "C1", "scenario": "Standard Scenario"}, {"value": "0.0", "module": "C2", "scenario": "Standard Scenario"}, {"value": "0.0", "module": "C3", "scenario": "Standard Scenario"}, {"value": "0.0", "module": "C4", "scenario": "Standard Scenario"}, {"value": "0.0", "module": "D", "scenario": "Standard Scenario"}, {"name": "referenceToUnitGroupDataSet", "value": {"shortDescription": [{"value": "MJ", "lang": "en"}], "type": "unit group data set", "refObjectId": "93a60a57-a3c8-11da-a746-0800200c9a66", "version": "03.00.000", "uri": "../unitgroups/93a60a57-a3c8-11da-a746-0800200c9a66.xml"}}]}, "flowProperties": [], "typeOfFlow": "Other flow", "classification": {"classHierarchy": "Größen / Umweltliche Größen / EPD EN 15804 / LCI Indikatoren", "name": "GaBiCategories"}}, {"dataSetInternalID": 11, "referenceToFlowDataSet": {"shortDescription": [{"value": "Use of non renewable primary energy (PENRE)", "lang": "en"}, {"value": "Nicht-erneuerbare Primärenergie als Energieträger (PENRE)", "lang": "de"}, {"value": "Uso de energía primaria no renovable, excluyendo los recursos de energía primaria no renovable utilizada como materia prima (PENRE)", "lang": "es"}], "type": "flow data set", "refObjectId": "ac857178-2b45-46ec-892a-a9a4332f0372", "version": "38.00.000", "uri": "../flows/ac857178-2b45-46ec-892a-a9a4332f0372.xml"}, "exchange direction": "INPUT", "meanAmount": 0.0, "other": {"anies": [{"value": "12.9256651007448", "module": "A1", "scenario": "Standard Scenario"}, {"value": "0.23710381957432", "module": "A2", "scenario": "Standard Scenario"}, {"value": "1.56861053919819", "module": "A3", "scenario": "Standard Scenario"}, {"value": "14.73137945951731", "module": "A1-A3", "scenario": "Standard Scenario"}, {"value": "0.83916120075784", "module": "A4", "scenario": "Standard Scenario"}, {"value": "0.84372741228284", "module": "A5", "scenario": "Standard Scenario"}, {"value": "0.0", "module": "B1", "scenario": "Standard Scenario"}, {"value": "0.0", "module": "B2", "scenario": "Standard Scenario"}, {"value": "0.0", "module": "B3", "scenario": "Standard Scenario"}, {"value": "0.0", "module": "B6", "scenario": "Standard Scenario"}, {"value": "0.0", "module": "B7", "scenario": "Standard Scenario"}, {"value": "0.0", "module": "C1", "scenario": "Standard Scenario"}, {"value": "0.09303673241807", "module": "C2", "scenario": "Standard Scenario"}, {"value": "0.56805828194122", "module": "C3", "scenario": "Standard Scenario"}, {"value": "0.00820445890028", "module": "C4", "scenario": "Standard Scenario"}, {"value": "-9.07675483099517", "module": "D", "scenario": "Standard Scenario"}, {"name": "referenceToUnitGroupDataSet", "value": {"shortDescription": [{"value": "MJ", "lang": "en"}], "type": "unit group data set", "refObjectId": "93a60a57-a3c8-11da-a746-0800200c9a66", "version": "03.00.000", "uri": "../unitgroups/93a60a57-a3c8-11da-a746-0800200c9a66.xml"}}]}, "flowProperties": [], "typeOfFlow": "Other flow", "classification": {"classHierarchy": "Quantities", "name": "GaBiCategories"}}, {"dataSetInternalID": 12, "referenceToFlowDataSet": {"shortDescription": [{"value": "Use of non renewable primary energy resources used as raw materials (PENRM)", "lang": "en"}, {"value": "Nicht-erneuerbare Primärenergie zur stofflichen Nutzung (PENRM)", "lang": "de"}, {"value": "Uso de la energía primaria no renovable utilizada como materia prima (PENRM)", "lang": "es"}], "type": "flow data set", "refObjectId": "1421caa0-679d-4bf4-b282-0eb850ccae27", "version": "38.00.000", "uri": "../flows/1421caa0-679d-4bf4-b282-0eb850ccae27.xml"}, "exchange direction": "INPUT", "meanAmount": 0.0, "other": {"anies": [{"value": "10.6324583028125", "module": "A1", "scenario": "Standard Scenario"}, {"value": "0.0", "module": "A2", "scenario": "Standard Scenario"}, {"value": "0.011144", "module": "A3", "scenario": "Standard Scenario"}, {"value": "10.6436023028125", "module": "A1-A3", "scenario": "Standard Scenario"}, {"value": "0.0", "module": "A4", "scenario": "Standard Scenario"}, {"value": "0.53218011514063", "module": "A5", "scenario": "Standard Scenario"}, {"value": "0.0", "module": "B1", "scenario": "Standard Scenario"}, {"value": "0.0", "module": "B2", "scenario": "Standard Scenario"}, {"value": "0.0", "module": "B3", "scenario": "Standard Scenario"}, {"value": "0.0", "module": "B6", "scenario": "Standard Scenario"}, {"value": "0.0", "module": "B7", "scenario": "Standard Scenario"}, {"value": "0.0", "module": "C1", "scenario": "Standard Scenario"}, {"value": "0.0", "module": "C2", "scenario": "Standard Scenario"}, {"value": "0.0", "module": "C3", "scenario": "Standard Scenario"}, {"value": "0.0", "module": "C4", "scenario": "Standard Scenario"}, {"value": "-0.45939577512314", "module": "D", "scenario": "Standard Scenario"}, {"name": "referenceToUnitGroupDataSet", "value": {"shortDescription": [{"value": "MJ", "lang": "en"}], "type": "unit group data set", "refObjectId": "93a60a57-a3c8-11da-a746-0800200c9a66", "version": "03.00.000", "uri": "../unitgroups/93a60a57-a3c8-11da-a746-0800200c9a66.xml"}}]}, "flowProperties": [], "typeOfFlow": "Other flow", "classification": {"classHierarchy": "Quantities", "name": "GaBiCategories"}}, {"dataSetInternalID": 13, "referenceToFlowDataSet": {"shortDescription": [{"value": "Total use of non-renewable primary energy resources (PENRT)", "lang": "en"}, {"value": "Total nicht erneuerbare Primärenergie (PENRT)", "lang": "de"}, {"value": "Uso total de la energía primaria no renovable (energía primaria y recursos de energía primaria renovable utilizada como materia prima) (PENRT)", "lang": "es"}], "type": "flow data set", "refObjectId": "06159210-646b-4c8d-8583-da9b3b95a6c1", "version": "30.00.000", "uri": "../flows/06159210-646b-4c8d-8583-da9b3b95a6c1.xml"}, "exchange direction": "INPUT", "meanAmount": 0.0, "other": {"anies": [{"value": "23.5581234035575", "module": "A1", "scenario": "Standard Scenario"}, {"value": "0.23710381957432", "module": "A2", "scenario": "Standard Scenario"}, {"value": "1.57975453919819", "module": "A3", "scenario": "Standard Scenario"}, {"value": "25.37498176233001", "module": "A1-A3", "scenario": "Standard Scenario"}, {"value": "0.83916120075784", "module": "A4", "scenario": "Standard Scenario"}, {"value": "1.37590752742347", "module": "A5", "scenario": "Standard Scenario"}, {"value": "0.0", "module": "B1", "scenario": "Standard Scenario"}, {"value": "0.0", "module": "B2", "scenario": "Standard Scenario"}, {"value": "0.0", "module": "B3", "scenario": "Standard Scenario"}, {"value": "0.0", "module": "B6", "scenario": "Standard Scenario"}, {"value": "0.0", "module": "B7", "scenario": "Standard Scenario"}, {"value": "0.0", "module": "C1", "scenario": "Standard Scenario"}, {"value": "0.09303673241807", "module": "C2", "scenario": "Standard Scenario"}, {"value": "0.56805828194122", "module": "C3", "scenario": "Standard Scenario"}, {"value": "0.00820445890028", "module": "C4", "scenario": "Standard Scenario"}, {"value": "-9.53615060611832", "module": "D", "scenario": "Standard Scenario"}, {"name": "referenceToUnitGroupDataSet", "value": {"shortDescription": [{"value": "MJ", "lang": "en"}], "type": "unit group data set", "refObjectId": "93a60a57-a3c8-11da-a746-0800200c9a66", "version": "03.00.000", "uri": "../unitgroups/93a60a57-a3c8-11da-a746-0800200c9a66.xml"}}]}, "flowProperties": [], "typeOfFlow": "Other flow", "classification": {"classHierarchy": "Größen / Umweltliche Größen / EPD EN 15804 / LCI Indikatoren", "name": "GaBiCategories"}}, {"dataSetInternalID": 14, "referenceToFlowDataSet": {"shortDescription": [{"value": "Use of renewable primary energy (PERE)", "lang": "en"}, {"value": "Erneuerbare Primärenergie als Energieträger (PERE)", "lang": "de"}, {"value": "Uso de energía primaria renovable excluyendo los recursos de energía primaria renovable utilizada como materia prima (PERE)", "lang": "es"}], "type": "flow data set", "refObjectId": "20f32be5-0398-4288-9b6d-accddd195317", "version": "38.00.000", "uri": "../flows/20f32be5-0398-4288-9b6d-accddd195317.xml"}, "exchange direction": "INPUT", "meanAmount": 0.0, "other": {"anies": [{"value": "0.62551450368211", "module": "A1", "scenario": "Standard Scenario"}, {"value": "0.00279580218078", "module": "A2", "scenario": "Standard Scenario"}, {"value": "0.18335899611482", "module": "A3", "scenario": "Standard Scenario"}, {"value": "0.81166930197771", "module": "A1-A3", "scenario": "Standard Scenario"}, {"value": "0.00989494272728", "module": "A4", "scenario": "Standard Scenario"}, {"value": "0.04488164621926", "module": "A5", "scenario": "Standard Scenario"}, {"value": "0.0", "module": "B1", "scenario": "Standard Scenario"}, {"value": "0.0", "module": "B2", "scenario": "Standard Scenario"}, {"value": "0.0", "module": "B3", "scenario": "Standard Scenario"}, {"value": "0.0", "module": "B6", "scenario": "Standard Scenario"}, {"value": "0.0", "module": "B7", "scenario": "Standard Scenario"}, {"value": "0.0", "module": "C1", "scenario": "Standard Scenario"}, {"value": "0.00109703968436", "module": "C2", "scenario": "Standard Scenario"}, {"value": "0.05472672932537", "module": "C3", "scenario": "Standard Scenario"}, {"value": "1.3659952336E-4", "module": "C4", "scenario": "Standard Scenario"}, {"value": "-0.65128858342751", "module": "D", "scenario": "Standard Scenario"}, {"name": "referenceToUnitGroupDataSet", "value": {"shortDescription": [{"value": "MJ", "lang": "en"}], "type": "unit group data set", "refObjectId": "93a60a57-a3c8-11da-a746-0800200c9a66", "version": "03.00.000", "uri": "../unitgroups/93a60a57-a3c8-11da-a746-0800200c9a66.xml"}}]}, "flowProperties": [], "typeOfFlow": "Other flow", "classification": {"classHierarchy": "Quantities", "name": "GaBiCategories"}}, {"dataSetInternalID": 15, "referenceToFlowDataSet": {"shortDescription": [{"value": "Use of renewable primary energy resources used as raw materials (PERM)", "lang": "en"}, {"value": "Erneuerbare Primärenergie zur stofflichen Nutzung (PERM)", "lang": "de"}, {"value": "Uso de energía primaria renovable utilizada como materia prima (PERM)", "lang": "es"}], "type": "flow data set", "refObjectId": "fb3ec0de-548d-4508-aea5-00b73bf6f702", "version": "38.00.000", "uri": "../flows/fb3ec0de-548d-4508-aea5-00b73bf6f702.xml"}, "exchange direction": "INPUT", "meanAmount": 0.0, "other": {"anies": [{"value": "0.0", "module": "A1", "scenario": "Standard Scenario"}, {"value": "0.0", "module": "A2", "scenario": "Standard Scenario"}, {"value": "0.692951", "module": "A3", "scenario": "Standard Scenario"}, {"value": "0.692951", "module": "A1-A3", "scenario": "Standard Scenario"}, {"value": "0.0", "module": "A4", "scenario": "Standard Scenario"}, {"value": "0.03464755", "module": "A5", "scenario": "Standard Scenario"}, {"value": "0.0", "module": "B1", "scenario": "Standard Scenario"}, {"value": "0.0", "module": "B2", "scenario": "Standard Scenario"}, {"value": "0.0", "module": "B3", "scenario": "Standard Scenario"}, {"value": "0.0", "module": "B6", "scenario": "Standard Scenario"}, {"value": "0.0", "module": "B7", "scenario": "Standard Scenario"}, {"value": "0.0", "module": "C1", "scenario": "Standard Scenario"}, {"value": "0.0", "module": "C2", "scenario": "Standard Scenario"}, {"value": "0.0", "module": "C3", "scenario": "Standard Scenario"}, {"value": "0.0", "module": "C4", "scenario": "Standard Scenario"}, {"value": "0.0", "module": "D", "scenario": "Standard Scenario"}, {"name": "referenceToUnitGroupDataSet", "value": {"shortDescription": [{"value": "MJ", "lang": "en"}], "type": "unit group data set", "refObjectId": "93a60a57-a3c8-11da-a746-0800200c9a66", "version": "03.00.000", "uri": "../unitgroups/93a60a57-a3c8-11da-a746-0800200c9a66.xml"}}]}, "flowProperties": [], "typeOfFlow": "Other flow", "classification": {"classHierarchy": "Quantities", "name": "GaBiCategories"}}, {"dataSetInternalID": 16, "referenceToFlowDataSet": {"shortDescription": [{"value": "Total use of renewable primary energy resources (PERT)", "lang": "en"}, {"value": "Total erneuerbare Primärenergie (PERT)", "lang": "de"}, {"value": "Uso total de la energía primaria renovable (energía primaria y recursos de energía primaria renovable utilizada como materia prima) (PERT)", "lang": "es"}], "type": "flow data set", "refObjectId": "53f97275-fa8a-4cdd-9024-65936002acd0", "version": "30.00.000", "uri": "../flows/53f97275-fa8a-4cdd-9024-65936002acd0.xml"}, "exchange direction": "INPUT", "meanAmount": 0.0, "other": {"anies": [{"value": "0.62551450368211", "module": "A1", "scenario": "Standard Scenario"}, {"value": "0.00279580218078", "module": "A2", "scenario": "Standard Scenario"}, {"value": "0.87630999611483", "module": "A3", "scenario": "Standard Scenario"}, {"value": "1.50462030197772", "module": "A1-A3", "scenario": "Standard Scenario"}, {"value": "0.00989494272728", "module": "A4", "scenario": "Standard Scenario"}, {"value": "0.07952919621926", "module": "A5", "scenario": "Standard Scenario"}, {"value": "0.0", "module": "B1", "scenario": "Standard Scenario"}, {"value": "0.0", "module": "B2", "scenario": "Standard Scenario"}, {"value": "0.0", "module": "B3", "scenario": "Standard Scenario"}, {"value": "0.0", "module": "B6", "scenario": "Standard Scenario"}, {"value": "0.0", "module": "B7", "scenario": "Standard Scenario"}, {"value": "0.0", "module": "C1", "scenario": "Standard Scenario"}, {"value": "0.00109703968436", "module": "C2", "scenario": "Standard Scenario"}, {"value": "0.05472672932537", "module": "C3", "scenario": "Standard Scenario"}, {"value": "1.3659952336E-4", "module": "C4", "scenario": "Standard Scenario"}, {"value": "-0.65128858342751", "module": "D", "scenario": "Standard Scenario"}, {"name": "referenceToUnitGroupDataSet", "value": {"shortDescription": [{"value": "MJ", "lang": "en"}], "type": "unit group data set", "refObjectId": "93a60a57-a3c8-11da-a746-0800200c9a66", "version": "03.00.000", "uri": "../unitgroups/93a60a57-a3c8-11da-a746-0800200c9a66.xml"}}]}, "flowProperties": [], "typeOfFlow": "Other flow", "classification": {"classHierarchy": "Größen / Umweltliche Größen / EPD EN 15804 / LCI Indikatoren", "name": "GaBiCategories"}}, {"dataSetInternalID": 17, "referenceToFlowDataSet": {"shortDescription": [{"value": "Use of renewable secondary fuels (RSF)", "lang": "en"}, {"value": "Erneuerbare Sekundärbrennstoffe (RSF)", "lang": "de"}, {"value": "Uso de combustibles secundarios renovables (RSF)", "lang": "es"}], "type": "flow data set", "refObjectId": "64333088-a55f-4aa2-9a31-c10b07816787", "version": "30.00.000", "uri": "../flows/64333088-a55f-4aa2-9a31-c10b07816787.xml"}, "exchange direction": "INPUT", "meanAmount": 0.0, "other": {"anies": [{"value": "0.0", "module": "A1", "scenario": "Standard Scenario"}, {"value": "0.0", "module": "A2", "scenario": "Standard Scenario"}, {"value": "0.0", "module": "A3", "scenario": "Standard Scenario"}, {"value": "0.0", "module": "A1-A3", "scenario": "Standard Scenario"}, {"value": "0.0", "module": "A4", "scenario": "Standard Scenario"}, {"value": "0.0", "module": "A5", "scenario": "Standard Scenario"}, {"value": "0.0", "module": "B1", "scenario": "Standard Scenario"}, {"value": "0.0", "module": "B2", "scenario": "Standard Scenario"}, {"value": "0.0", "module": "B3", "scenario": "Standard Scenario"}, {"value": "0.0", "module": "B6", "scenario": "Standard Scenario"}, {"value": "0.0", "module": "B7", "scenario": "Standard Scenario"}, {"value": "0.0", "module": "C1", "scenario": "Standard Scenario"}, {"value": "0.0", "module": "C2", "scenario": "Standard Scenario"}, {"value": "0.0", "module": "C3", "scenario": "Standard Scenario"}, {"value": "0.0", "module": "C4", "scenario": "Standard Scenario"}, {"value": "0.0", "module": "D", "scenario": "Standard Scenario"}, {"name": "referenceToUnitGroupDataSet", "value": {"shortDescription": [{"value": "MJ", "lang": "en"}], "type": "unit group data set", "refObjectId": "93a60a57-a3c8-11da-a746-0800200c9a66", "version": "03.00.000", "uri": "../unitgroups/93a60a57-a3c8-11da-a746-0800200c9a66.xml"}}]}, "flowProperties": [], "typeOfFlow": "Other flow", "classification": {"classHierarchy": "Größen / Umweltliche Größen / EPD EN 15804 / LCI Indikatoren", "name": "GaBiCategories"}}, {"dataSetInternalID": 18, "referenceToFlowDataSet": {"shortDescription": [{"value": "Radioactive waste disposed (RWD)", "lang": "en"}, {"value": "Entsorgter radioaktiver Abfall (RWD)", "lang": "de"}, {"value": "Residuos radiactivos eliminados (RWD)", "lang": "es"}], "type": "flow data set", "refObjectId": "3449546e-52ad-4b39-b809-9fb77cea8ff6", "version": "30.00.000", "uri": "../flows/3449546e-52ad-4b39-b809-9fb77cea8ff6.xml"}, "exchange direction": "OUTPUT", "meanAmount": 0.0, "other": {"anies": [{"value": "2.072615688E-5", "module": "A1", "scenario": "Standard Scenario"}, {"value": "1.46644892E-6", "module": "A2", "scenario": "Standard Scenario"}, {"value": "1.162103037E-5", "module": "A3", "scenario": "Standard Scenario"}, {"value": "3.3813636169999996E-5", "module": "A1-A3", "scenario": "Standard Scenario"}, {"value": "5.1900768E-6", "module": "A4", "scenario": "Standard Scenario"}, {"value": "2.26163721E-6", "module": "A5", "scenario": "Standard Scenario"}, {"value": "0.0", "module": "B1", "scenario": "Standard Scenario"}, {"value": "0.0", "module": "B2", "scenario": "Standard Scenario"}, {"value": "0.0", "module": "B3", "scenario": "Standard Scenario"}, {"value": "0.0", "module": "B6", "scenario": "Standard Scenario"}, {"value": "0.0", "module": "B7", "scenario": "Standard Scenario"}, {"value": "0.0", "module": "C1", "scenario": "Standard Scenario"}, {"value": "5.754172E-7", "module": "C2", "scenario": "Standard Scenario"}, {"value": "1.92060406E-6", "module": "C3", "scenario": "Standard Scenario"}, {"value": "4.582019E-8", "module": "C4", "scenario": "Standard Scenario"}, {"value": "-4.35293166E-6", "module": "D", "scenario": "Standard Scenario"}, {"name": "referenceToUnitGroupDataSet", "value": {"shortDescription": [{"value": "kg", "lang": "en"}], "type": "unit group data set", "refObjectId": "ad38d542-3fe9-439d-9b95-2f5f7752acaf", "version": "30.00.000", "uri": "../unitgroups/ad38d542-3fe9-439d-9b95-2f5f7752acaf.xml"}}]}, "flowProperties": [], "typeOfFlow": "Other flow", "classification": {"classHierarchy": "Größen / Umweltliche Größen / EPD EN 15804 / LCI Indikatoren", "name": "GaBiCategories"}}, {"dataSetInternalID": 19, "referenceToFlowDataSet": {"shortDescription": [{"value": "Use of secondary material (SM)", "lang": "en"}, {"value": "Einsatz von Sekundärstoffen (SM)", "lang": "de"}, {"value": "Uso de materiales secundarios (SM)", "lang": "es"}], "type": "flow data set", "refObjectId": "c6a1f35f-2d09-4f54-8dfb-97e502e1ce92", "version": "30.00.000", "uri": "../flows/c6a1f35f-2d09-4f54-8dfb-97e502e1ce92.xml"}, "exchange direction": "INPUT", "meanAmount": 0.0, "other": {"anies": [{"value": "0.0", "module": "A1", "scenario": "Standard Scenario"}, {"value": "0.0", "module": "A2", "scenario": "Standard Scenario"}, {"value": "0.0", "module": "A3", "scenario": "Standard Scenario"}, {"value": "0.0", "module": "A1-A3", "scenario": "Standard Scenario"}, {"value": "0.0", "module": "A4", "scenario": "Standard Scenario"}, {"value": "0.0", "module": "A5", "scenario": "Standard Scenario"}, {"value": "0.0", "module": "B1", "scenario": "Standard Scenario"}, {"value": "0.0", "module": "B2", "scenario": "Standard Scenario"}, {"value": "0.0", "module": "B3", "scenario": "Standard Scenario"}, {"value": "0.0", "module": "B6", "scenario": "Standard Scenario"}, {"value": "0.0", "module": "B7", "scenario": "Standard Scenario"}, {"value": "0.0", "module": "C1", "scenario": "Standard Scenario"}, {"value": "0.0", "module": "C2", "scenario": "Standard Scenario"}, {"value": "0.0", "module": "C3", "scenario": "Standard Scenario"}, {"value": "0.0", "module": "C4", "scenario": "Standard Scenario"}, {"value": "0.0", "module": "D", "scenario": "Standard Scenario"}, {"name": "referenceToUnitGroupDataSet", "value": {"shortDescription": [{"value": "kg", "lang": "en"}], "type": "unit group data set", "refObjectId": "ad38d542-3fe9-439d-9b95-2f5f7752acaf", "version": "30.00.000", "uri": "../unitgroups/ad38d542-3fe9-439d-9b95-2f5f7752acaf.xml"}}]}, "flowProperties": [], "typeOfFlow": "Other flow", "classification": {"classHierarchy": "Größen / Umweltliche Größen / EPD EN 15804 / LCI Indikatoren", "name": "GaBiCategories"}}]}, "LCIAResults": {"LCIAResult": [{"referenceToLCIAMethodDataSet": {"shortDescription": [{"value": "Abiotic depletion potential - non-fossil resources (ADPE)", "lang": "en"}, {"value": "Potenzial für die Verknappung abiotischer Ressourcen – nicht fossile Ressourcen (ADPE)", "lang": "de"}], "type": "LCIA method data set", "refObjectId": "b2ad6494-c78d-11e6-9d9d-cec0c932ce01", "version": "01.00.011", "uri": "../lciamethods/b2ad6494-c78d-11e6-9d9d-cec0c932ce01.xml"}, "meanAmount": 0.0, "other": {"anies": [{"value": "5.73591825E-6", "module": "A1", "scenario": "Standard Scenario"}, {"value": "3.7516524E-7", "module": "A2", "scenario": "Standard Scenario"}, {"value": "9.1177132E-7", "module": "A3", "scenario": "Standard Scenario"}, {"value": "7.02285481E-6", "module": "A1-A3", "scenario": "Standard Scenario"}, {"value": "1.32779015E-6", "module": "A4", "scenario": "Standard Scenario"}, {"value": "5.3983343E-7", "module": "A5", "scenario": "Standard Scenario"}, {"value": "0.0", "module": "B1", "scenario": "Standard Scenario"}, {"value": "0.0", "module": "B2", "scenario": "Standard Scenario"}, {"value": "0.0", "module": "B3", "scenario": "Standard Scenario"}, {"value": "0.0", "module": "B6", "scenario": "Standard Scenario"}, {"value": "0.0", "module": "B7", "scenario": "Standard Scenario"}, {"value": "0.0", "module": "C1", "scenario": "Standard Scenario"}, {"value": "1.472104E-7", "module": "C2", "scenario": "Standard Scenario"}, {"value": "8.853445E-7", "module": "C3", "scenario": "Standard Scenario"}, {"value": "3.47495E-9", "module": "C4", "scenario": "Standard Scenario"}, {"value": "-3.4676845E-7", "module": "D", "scenario": "Standard Scenario"}, {"name": "referenceToUnitGroupDataSet", "value": {"shortDescription": [{"value": "kg Sb-eq.", "lang": "en"}], "type": "unit group data set", "refObjectId": "54ccd2d9-a32a-4fc2-923d-f2c8c93e89d4", "version": "30.00.000", "uri": "../unitgroups/54ccd2d9-a32a-4fc2-923d-f2c8c93e89d4.xml"}}]}}, {"referenceToLCIAMethodDataSet": {"shortDescription": [{"value": "Abiotic depletion potential - fossil resources (ADPF)", "lang": "en"}, {"value": "Potenzial für die Verknappung abiotischer Ressourcen – fossile Brennstoffe (ADPF)", "lang": "de"}], "type": "LCIA method data set", "refObjectId": "b2ad6110-c78d-11e6-9d9d-cec0c932ce01", "version": "01.00.011", "uri": "../lciamethods/b2ad6110-c78d-11e6-9d9d-cec0c932ce01.xml"}, "meanAmount": 0.0, "other": {"anies": [{"value": "21.9878808738036", "module": "A1", "scenario": "Standard Scenario"}, {"value": "0.22331956952247", "module": "A2", "scenario": "Standard Scenario"}, {"value": "1.5184540712363", "module": "A3", "scenario": "Standard Scenario"}, {"value": "23.72965451456237", "module": "A1-A3", "scenario": "Standard Scenario"}, {"value": "0.79037578749109", "module": "A4", "scenario": "Standard Scenario"}, {"value": "1.28738358267337", "module": "A5", "scenario": "Standard Scenario"}, {"value": "0.0", "module": "B1", "scenario": "Standard Scenario"}, {"value": "0.0", "module": "B2", "scenario": "Standard Scenario"}, {"value": "0.0", "module": "B3", "scenario": "Standard Scenario"}, {"value": "0.0", "module": "B6", "scenario": "Standard Scenario"}, {"value": "0.0", "module": "B7", "scenario": "Standard Scenario"}, {"value": "0.0", "module": "C1", "scenario": "Standard Scenario"}, {"value": "0.08762795584938", "module": "C2", "scenario": "Standard Scenario"}, {"value": "0.53450538591533", "module": "C3", "scenario": "Standard Scenario"}, {"value": "0.00771953366752", "module": "C4", "scenario": "Standard Scenario"}, {"value": "-8.62266971385864", "module": "D", "scenario": "Standard Scenario"}, {"name": "referenceToUnitGroupDataSet", "value": {"shortDescription": [{"value": "MJ", "lang": "en"}], "type": "unit group data set", "refObjectId": "93a60a57-a3c8-11da-a746-0800200c9a66", "version": "03.00.000", "uri": "../unitgroups/93a60a57-a3c8-11da-a746-0800200c9a66.xml"}}]}}, {"referenceToLCIAMethodDataSet": {"shortDescription": [{"value": "Acidification potential, Accumulated Exceedance (AP)", "lang": "en"}, {"value": "Versauerungspotenzial, kumulierte Überschreitung (AP)", "lang": "de"}], "type": "LCIA method data set", "refObjectId": "b5c611c6-def3-11e6-bf01-fe55135034f3", "version": "01.03.010", "uri": "../lciamethods/b5c611c6-def3-11e6-bf01-fe55135034f3.xml"}, "meanAmount": 0.0, "other": {"anies": [{"value": "0.00247218929538", "module": "A1", "scenario": "Standard Scenario"}, {"value": "8.587690586E-5", "module": "A2", "scenario": "Standard Scenario"}, {"value": "5.0721560992E-4", "module": "A3", "scenario": "Standard Scenario"}, {"value": "0.00306528181116", "module": "A1-A3", "scenario": "Standard Scenario"}, {"value": "3.039367631E-4", "module": "A4", "scenario": "Standard Scenario"}, {"value": "2.0488430791E-4", "module": "A5", "scenario": "Standard Scenario"}, {"value": "0.0", "module": "B1", "scenario": "Standard Scenario"}, {"value": "0.0", "module": "B2", "scenario": "Standard Scenario"}, {"value": "0.0", "module": "B3", "scenario": "Standard Scenario"}, {"value": "0.0", "module": "B6", "scenario": "Standard Scenario"}, {"value": "0.0", "module": "B7", "scenario": "Standard Scenario"}, {"value": "0.0", "module": "C1", "scenario": "Standard Scenario"}, {"value": "3.369708141E-5", "module": "C2", "scenario": "Standard Scenario"}, {"value": "3.1269974185E-4", "module": "C3", "scenario": "Standard Scenario"}, {"value": "2.84454208E-6", "module": "C4", "scenario": "Standard Scenario"}, {"value": "-5.0259798734E-4", "module": "D", "scenario": "Standard Scenario"}, {"name": "referenceToUnitGroupDataSet", "value": {"shortDescription": [{"value": "mol H+-eq.", "lang": "en"}], "type": "unit group data set", "refObjectId": "42e089ac-92bf-4bf2-8ca1-5fc40d18f2ed", "version": "00.01.000", "uri": "../unitgroups/42e089ac-92bf-4bf2-8ca1-5fc40d18f2ed.xml"}}]}}, {"referenceToLCIAMethodDataSet": {"shortDescription": [{"value": "Eutrophication potential - freshwater (EP-freshwater)", "lang": "en"}, {"value": "Eutrophierungspotenzial - Süßwasser (EP-freshwater)", "lang": "de"}], "type": "LCIA method data set", "refObjectId": "b53ec18f-7377-4ad3-86eb-cc3f4f276b2b", "version": "01.00.011", "uri": "../lciamethods/b53ec18f-7377-4ad3-86eb-cc3f4f276b2b.xml"}, "meanAmount": 0.0, "other": {"anies": [{"value": "1.758061731E-5", "module": "A1", "scenario": "Standard Scenario"}, {"value": "1.4936798E-7", "module": "A2", "scenario": "Standard Scenario"}, {"value": "8.81470815E-6", "module": "A3", "scenario": "Standard Scenario"}, {"value": "2.6544693439999997E-5", "module": "A1-A3", "scenario": "Standard Scenario"}, {"value": "5.2864527E-7", "module": "A4", "scenario": "Standard Scenario"}, {"value": "1.50203689E-6", "module": "A5", "scenario": "Standard Scenario"}, {"value": "0.0", "module": "B1", "scenario": "Standard Scenario"}, {"value": "0.0", "module": "B2", "scenario": "Standard Scenario"}, {"value": "0.0", "module": "B3", "scenario": "Standard Scenario"}, {"value": "0.0", "module": "B6", "scenario": "Standard Scenario"}, {"value": "0.0", "module": "B7", "scenario": "Standard Scenario"}, {"value": "0.0", "module": "C1", "scenario": "Standard Scenario"}, {"value": "5.861023E-8", "module": "C2", "scenario": "Standard Scenario"}, {"value": "2.09465928E-6", "module": "C3", "scenario": "Standard Scenario"}, {"value": "5.84284E-9", "module": "C4", "scenario": "Standard Scenario"}, {"value": "-1.08741081E-6", "module": "D", "scenario": "Standard Scenario"}, {"name": "referenceToUnitGroupDataSet", "value": {"shortDescription": [{"value": "kg P-eq.", "lang": "en"}], "type": "unit group data set", "refObjectId": "0429039d-a61d-4590-ba67-aa4a20a810a1", "version": "30.00.000", "uri": "../unitgroups/0429039d-a61d-4590-ba67-aa4a20a810a1.xml"}}]}}, {"referenceToLCIAMethodDataSet": {"shortDescription": [{"value": "Eutrophication potential - marine (EP-marine)", "lang": "en"}, {"value": "Eutrophierungspotenzial - Salzwasser (EP-marine)", "lang": "de"}], "type": "LCIA method data set", "refObjectId": "b5c619fa-def3-11e6-bf01-fe55135034f3", "version": "02.00.011", "uri": "../lciamethods/b5c619fa-def3-11e6-bf01-fe55135034f3.xml"}, "meanAmount": 0.0, "other": {"anies": [{"value": "4.1676784982E-4", "module": "A1", "scenario": "Standard Scenario"}, {"value": "3.026096222E-5", "module": "A2", "scenario": "Standard Scenario"}, {"value": "1.09581003E-4", "module": "A3", "scenario": "Standard Scenario"}, {"value": "5.5660981504E-4", "module": "A1-A3", "scenario": "Standard Scenario"}, {"value": "1.0710002663E-4", "module": "A4", "scenario": "Standard Scenario"}, {"value": "4.550471217E-5", "module": "A5", "scenario": "Standard Scenario"}, {"value": "0.0", "module": "B1", "scenario": "Standard Scenario"}, {"value": "0.0", "module": "B2", "scenario": "Standard Scenario"}, {"value": "0.0", "module": "B3", "scenario": "Standard Scenario"}, {"value": "0.0", "module": "B6", "scenario": "Standard Scenario"}, {"value": "0.0", "module": "B7", "scenario": "Standard Scenario"}, {"value": "0.0", "module": "C1", "scenario": "Standard Scenario"}, {"value": "1.18740434E-5", "module": "C2", "scenario": "Standard Scenario"}, {"value": "8.552077318E-5", "module": "C3", "scenario": "Standard Scenario"}, {"value": "1.72210115E-6", "module": "C4", "scenario": "Standard Scenario"}, {"value": "-1.4087923378E-4", "module": "D", "scenario": "Standard Scenario"}, {"name": "referenceToUnitGroupDataSet", "value": {"shortDescription": [{"value": "kg N-eq.", "lang": "en"}], "type": "unit group data set", "refObjectId": "d05bb823-ecdf-4686-8c40-bf1d9257859f", "version": "00.00.003", "uri": "../unitgroups/d05bb823-ecdf-4686-8c40-bf1d9257859f.xml"}}]}}, {"referenceToLCIAMethodDataSet": {"shortDescription": [{"value": "Eutrophication potential - terrestrial (EP-terrestrial)", "lang": "en"}, {"value": "Eutrophierungspotenzial - Land (EP-terrestrial)", "lang": "de"}], "type": "LCIA method data set", "refObjectId": "b5c614d2-def3-11e6-bf01-fe55135034f3", "version": "01.02.010", "uri": "../lciamethods/b5c614d2-def3-11e6-bf01-fe55135034f3.xml"}, "meanAmount": 0.0, "other": {"anies": [{"value": "0.00469122853273", "module": "A1", "scenario": "Standard Scenario"}, {"value": "3.3363064259E-4", "module": "A2", "scenario": "Standard Scenario"}, {"value": "0.00104506819186", "module": "A3", "scenario": "Standard Scenario"}, {"value": "0.00606992736718", "module": "A1-A3", "scenario": "Standard Scenario"}, {"value": "0.0011807903017", "module": "A4", "scenario": "Standard Scenario"}, {"value": "4.9758002274E-4", "module": "A5", "scenario": "Standard Scenario"}, {"value": "0.0", "module": "B1", "scenario": "Standard Scenario"}, {"value": "0.0", "module": "B2", "scenario": "Standard Scenario"}, {"value": "0.0", "module": "B3", "scenario": "Standard Scenario"}, {"value": "0.0", "module": "B6", "scenario": "Standard Scenario"}, {"value": "0.0", "module": "B7", "scenario": "Standard Scenario"}, {"value": "0.0", "module": "C1", "scenario": "Standard Scenario"}, {"value": "1.3091271527E-4", "module": "C2", "scenario": "Standard Scenario"}, {"value": "9.5179915524E-4", "module": "C3", "scenario": "Standard Scenario"}, {"value": "1.045561413E-5", "module": "C4", "scenario": "Standard Scenario"}, {"value": "-0.00160775205785", "module": "D", "scenario": "Standard Scenario"}, {"name": "referenceToUnitGroupDataSet", "value": {"shortDescription": [{"value": "mol N-eq.", "lang": "en"}], "type": "unit group data set", "refObjectId": "71b4d617-0ec9-4d3f-b65e-e438940c2401", "version": "00.00.003", "uri": "../unitgroups/71b4d617-0ec9-4d3f-b65e-e438940c2401.xml"}}]}}, {"referenceToLCIAMethodDataSet": {"shortDescription": [{"value": "Potential Comparative Toxic Unit for ecosystems (ETP-fw)", "lang": "en"}, {"value": "Potenzielle Toxizitätsvergleichseinheit für Ökosysteme (ETP-fw)", "lang": "de"}], "type": "LCIA method data set", "refObjectId": "ee1082d1-b0f7-43ca-a1f0-21e2a4a74511", "version": "01.00.003", "uri": "../lciamethods/ee1082d1-b0f7-43ca-a1f0-21e2a4a74511.xml"}, "meanAmount": 0.0, "other": {"anies": [{"value": "4.08909605059095", "module": "A1", "scenario": "Standard Scenario"}, {"value": "0.19913877794039", "module": "A2", "scenario": "Standard Scenario"}, {"value": "1.29319120182657", "module": "A3", "scenario": "Standard Scenario"}, {"value": "5.5814260303579095", "module": "A1-A3", "scenario": "Standard Scenario"}, {"value": "0.70479478700059", "module": "A4", "scenario": "Standard Scenario"}, {"value": "0.8235581578804", "module": "A5", "scenario": "Standard Scenario"}, {"value": "0.0", "module": "B1", "scenario": "Standard Scenario"}, {"value": "0.0", "module": "B2", "scenario": "Standard Scenario"}, {"value": "0.0", "module": "B3", "scenario": "Standard Scenario"}, {"value": "0.0", "module": "B6", "scenario": "Standard Scenario"}, {"value": "0.0", "module": "B7", "scenario": "Standard Scenario"}, {"value": "0.0", "module": "C1", "scenario": "Standard Scenario"}, {"value": "0.07813969943868", "module": "C2", "scenario": "Standard Scenario"}, {"value": "8.8012200878712", "module": "C3", "scenario": "Standard Scenario"}, {"value": "0.00821020948804", "module": "C4", "scenario": "Standard Scenario"}, {"value": "-0.95047238864433", "module": "D", "scenario": "Standard Scenario"}, {"name": "referenceToUnitGroupDataSet", "value": {"shortDescription": [{"value": "CTUe", "lang": "en"}], "type": "unit group data set", "refObjectId": "aa959ded-f1eb-4efb-9c5c-2d60be36b3e6", "version": "00.00.003", "uri": "../unitgroups/aa959ded-f1eb-4efb-9c5c-2d60be36b3e6.xml"}}]}}, {"referenceToLCIAMethodDataSet": {"shortDescription": [{"value": "Global Warming Potential - biogenic (GWP-biogenic)", "lang": "en"}, {"value": "Globales Erwärmungspotenzial - biogen (GWP-biogenic)", "lang": "de"}], "type": "LCIA method data set", "refObjectId": "2356e1ab-0185-4db5-86e5-16de51c7485c", "version": "01.00.006", "uri": "../lciamethods/2356e1ab-0185-4db5-86e5-16de51c7485c.xml"}, "meanAmount": 0.0, "other": {"anies": [{"value": "8.2880236832E-4", "module": "A1", "scenario": "Standard Scenario"}, {"value": "6.83564994E-6", "module": "A2", "scenario": "Standard Scenario"}, {"value": "-0.07232413340737", "module": "A3", "scenario": "Standard Scenario"}, {"value": "-0.07148849538911", "module": "A1-A3", "scenario": "Standard Scenario"}, {"value": "2.419282919E-5", "module": "A4", "scenario": "Standard Scenario"}, {"value": "0.07493206292768", "module": "A5", "scenario": "Standard Scenario"}, {"value": "0.0", "module": "B1", "scenario": "Standard Scenario"}, {"value": "0.0", "module": "B2", "scenario": "Standard Scenario"}, {"value": "0.0", "module": "B3", "scenario": "Standard Scenario"}, {"value": "0.0", "module": "B6", "scenario": "Standard Scenario"}, {"value": "0.0", "module": "B7", "scenario": "Standard Scenario"}, {"value": "0.0", "module": "C1", "scenario": "Standard Scenario"}, {"value": "2.68222813E-6", "module": "C2", "scenario": "Standard Scenario"}, {"value": "1.0649350504E-4", "module": "C3", "scenario": "Standard Scenario"}, {"value": "3.50570591E-6", "module": "C4", "scenario": "Standard Scenario"}, {"value": "-1.1290951793E-4", "module": "D", "scenario": "Standard Scenario"}, {"name": "referenceToUnitGroupDataSet", "value": {"shortDescription": [{"value": "kg CO2-eq.", "lang": "en"}], "type": "unit group data set", "refObjectId": "1ebf3012-d0db-4de2-aefd-ef30cedb0be1", "version": "30.00.000", "uri": "../unitgroups/1ebf3012-d0db-4de2-aefd-ef30cedb0be1.xml"}}]}}, {"referenceToLCIAMethodDataSet": {"shortDescription": [{"value": "Global Warming Potential - fossil fuels (GWP-fossil)", "lang": "en"}, {"value": "Globales Erwärmungspotenzial - fossil (GWP-fossil)", "lang": "de"}], "type": "LCIA method data set", "refObjectId": "5f635281-343e-44fb-83df-1971b155e6b6", "version": "01.00.009", "uri": "../lciamethods/5f635281-343e-44fb-83df-1971b155e6b6.xml"}, "meanAmount": 0.0, "other": {"anies": [{"value": "0.63859457726961", "module": "A1", "scenario": "Standard Scenario"}, {"value": "0.01480703561732", "module": "A2", "scenario": "Standard Scenario"}, {"value": "0.06421192574033", "module": "A3", "scenario": "Standard Scenario"}, {"value": "0.71761353862726", "module": "A1-A3", "scenario": "Standard Scenario"}, {"value": "0.05240527044483", "module": "A4", "scenario": "Standard Scenario"}, {"value": "0.07658988747279", "module": "A5", "scenario": "Standard Scenario"}, {"value": "0.0", "module": "B1", "scenario": "Standard Scenario"}, {"value": "0.0", "module": "B2", "scenario": "Standard Scenario"}, {"value": "0.0", "module": "B3", "scenario": "Standard Scenario"}, {"value": "0.0", "module": "B6", "scenario": "Standard Scenario"}, {"value": "0.0", "module": "B7", "scenario": "Standard Scenario"}, {"value": "0.0", "module": "C1", "scenario": "Standard Scenario"}, {"value": "0.00581010551878", "module": "C2", "scenario": "Standard Scenario"}, {"value": "0.69992199638941", "module": "C3", "scenario": "Standard Scenario"}, {"value": "0.00456018534881", "module": "C4", "scenario": "Standard Scenario"}, {"value": "-0.49214176416676", "module": "D", "scenario": "Standard Scenario"}, {"name": "referenceToUnitGroupDataSet", "value": {"shortDescription": [{"value": "kg CO2-eq.", "lang": "en"}], "type": "unit group data set", "refObjectId": "1ebf3012-d0db-4de2-aefd-ef30cedb0be1", "version": "30.00.000", "uri": "../unitgroups/1ebf3012-d0db-4de2-aefd-ef30cedb0be1.xml"}}]}}, {"referenceToLCIAMethodDataSet": {"shortDescription": [{"value": "Global Warming Potential - land use and land use change (GWP-luluc)", "lang": "en"}, {"value": "Globales Erwärmungspotenzial - luluc (GWP-luluc)", "lang": "de"}], "type": "LCIA method data set", "refObjectId": "4331bbdb-978a-490d-8707-eeb047f01a55", "version": "01.00.006", "uri": "../lciamethods/4331bbdb-978a-490d-8707-eeb047f01a55.xml"}, "meanAmount": 0.0, "other": {"anies": [{"value": "3.3968596315E-4", "module": "A1", "scenario": "Standard Scenario"}, {"value": "5.42579706E-6", "module": "A2", "scenario": "Standard Scenario"}, {"value": "8.3121293754E-4", "module": "A3", "scenario": "Standard Scenario"}, {"value": "0.00117632469775", "module": "A1-A3", "scenario": "Standard Scenario"}, {"value": "1.920305789E-5", "module": "A4", "scenario": "Standard Scenario"}, {"value": "6.360893119E-5", "module": "A5", "scenario": "Standard Scenario"}, {"value": "0.0", "module": "B1", "scenario": "Standard Scenario"}, {"value": "0.0", "module": "B2", "scenario": "Standard Scenario"}, {"value": "0.0", "module": "B3", "scenario": "Standard Scenario"}, {"value": "0.0", "module": "B6", "scenario": "Standard Scenario"}, {"value": "0.0", "module": "B7", "scenario": "Standard Scenario"}, {"value": "0.0", "module": "C1", "scenario": "Standard Scenario"}, {"value": "2.12901854E-6", "module": "C2", "scenario": "Standard Scenario"}, {"value": "5.629118134E-5", "module": "C3", "scenario": "Standard Scenario"}, {"value": "1.6113946E-7", "module": "C4", "scenario": "Standard Scenario"}, {"value": "-4.81958408E-5", "module": "D", "scenario": "Standard Scenario"}, {"name": "referenceToUnitGroupDataSet", "value": {"shortDescription": [{"value": "kg CO2-eq.", "lang": "en"}], "type": "unit group data set", "refObjectId": "1ebf3012-d0db-4de2-aefd-ef30cedb0be1", "version": "30.00.000", "uri": "../unitgroups/1ebf3012-d0db-4de2-aefd-ef30cedb0be1.xml"}}]}}, {"referenceToLCIAMethodDataSet": {"shortDescription": [{"value": "Global Warming Potential - total (GWP-total)", "lang": "en"}, {"value": "Globales Erwärmungspotenzial - total (GWP-total)", "lang": "de"}], "type": "LCIA method data set", "refObjectId": "6a37f984-a4b3-458a-a20a-64418c145fa2", "version": "04.00.017", "uri": "../lciamethods/6a37f984-a4b3-458a-a20a-64418c145fa2.xml"}, "meanAmount": 0.0, "other": {"anies": [{"value": "0.63976306283831", "module": "A1", "scenario": "Standard Scenario"}, {"value": "0.01481929706431", "module": "A2", "scenario": "Standard Scenario"}, {"value": "-0.00728097338108", "module": "A3", "scenario": "Standard Scenario"}, {"value": "0.6473013865215399", "module": "A1-A3", "scenario": "Standard Scenario"}, {"value": "0.05244866633191", "module": "A4", "scenario": "Standard Scenario"}, {"value": "0.15158555697142", "module": "A5", "scenario": "Standard Scenario"}, {"value": "0.0", "module": "B1", "scenario": "Standard Scenario"}, {"value": "0.0", "module": "B2", "scenario": "Standard Scenario"}, {"value": "0.0", "module": "B3", "scenario": "Standard Scenario"}, {"value": "0.0", "module": "B6", "scenario": "Standard Scenario"}, {"value": "0.0", "module": "B7", "scenario": "Standard Scenario"}, {"value": "0.0", "module": "C1", "scenario": "Standard Scenario"}, {"value": "0.00581491676546", "module": "C2", "scenario": "Standard Scenario"}, {"value": "0.70008473494809", "module": "C3", "scenario": "Standard Scenario"}, {"value": "0.00456387556556", "module": "C4", "scenario": "Standard Scenario"}, {"value": "-0.4923028700829", "module": "D", "scenario": "Standard Scenario"}, {"name": "referenceToUnitGroupDataSet", "value": {"shortDescription": [{"value": "kg CO2-eq.", "lang": "en"}], "type": "unit group data set", "refObjectId": "1ebf3012-d0db-4de2-aefd-ef30cedb0be1", "version": "30.00.000", "uri": "../unitgroups/1ebf3012-d0db-4de2-aefd-ef30cedb0be1.xml"}}]}}, {"referenceToLCIAMethodDataSet": {"shortDescription": [{"value": "Potential Comparative Toxic Unit for humans - cancer effects (HTP-c)", "lang": "en"}, {"value": "Potenzielle Toxizitätsvergleichseinheit für den Menschen - kanzerogene Wirkung (HTP-c)", "lang": "de"}], "type": "LCIA method data set", "refObjectId": "2299222a-bbd8-474f-9d4f-4dd1f18aea7c", "version": "01.00.004", "uri": "../lciamethods/2299222a-bbd8-474f-9d4f-4dd1f18aea7c.xml"}, "meanAmount": 0.0, "other": {"anies": [{"value": "1.667E-10", "module": "A1", "scenario": "Standard Scenario"}, {"value": "6.46E-12", "module": "A2", "scenario": "Standard Scenario"}, {"value": "4.506E-11", "module": "A3", "scenario": "Standard Scenario"}, {"value": "2.1822E-10", "module": "A1-A3", "scenario": "Standard Scenario"}, {"value": "2.286E-11", "module": "A4", "scenario": "Standard Scenario"}, {"value": "2.637E-11", "module": "A5", "scenario": "Standard Scenario"}, {"value": "0.0", "module": "B1", "scenario": "Standard Scenario"}, {"value": "0.0", "module": "B2", "scenario": "Standard Scenario"}, {"value": "0.0", "module": "B3", "scenario": "Standard Scenario"}, {"value": "0.0", "module": "B6", "scenario": "Standard Scenario"}, {"value": "0.0", "module": "B7", "scenario": "Standard Scenario"}, {"value": "0.0", "module": "C1", "scenario": "Standard Scenario"}, {"value": "2.53E-12", "module": "C2", "scenario": "Standard Scenario"}, {"value": "1.3303E-10", "module": "C3", "scenario": "Standard Scenario"}, {"value": "2.2E-13", "module": "C4", "scenario": "Standard Scenario"}, {"value": "-4.0E-11", "module": "D", "scenario": "Standard Scenario"}, {"name": "referenceToUnitGroupDataSet", "value": {"shortDescription": [{"value": "CTUh", "lang": "en"}], "type": "unit group data set", "refObjectId": "d4c9523e-2d7e-49fd-8469-998f547d3a70", "version": "00.00.003", "uri": "../unitgroups/d4c9523e-2d7e-49fd-8469-998f547d3a70.xml"}}]}}, {"referenceToLCIAMethodDataSet": {"shortDescription": [{"value": "Potential Comparative Toxic Unit for humans - non-cancer effects (HTP-nc)", "lang": "en"}, {"value": "Potenzielle Toxizitätsvergleichseinheit für den Menschen - nicht kanzerogene Wirkung (HTP-nc)", "lang": "de"}], "type": "LCIA method data set", "refObjectId": "3af763a5-b7a1-48c9-9cee-1f223481fcef", "version": "01.00.003", "uri": "../lciamethods/3af763a5-b7a1-48c9-9cee-1f223481fcef.xml"}, "meanAmount": 0.0, "other": {"anies": [{"value": "4.39837E-9", "module": "A1", "scenario": "Standard Scenario"}, {"value": "2.1783E-10", "module": "A2", "scenario": "Standard Scenario"}, {"value": "1.289E-9", "module": "A3", "scenario": "Standard Scenario"}, {"value": "5.905200000000001E-9", "module": "A1-A3", "scenario": "Standard Scenario"}, {"value": "7.7094E-10", "module": "A4", "scenario": "Standard Scenario"}, {"value": "5.3835E-10", "module": "A5", "scenario": "Standard Scenario"}, {"value": "0.0", "module": "B1", "scenario": "Standard Scenario"}, {"value": "0.0", "module": "B2", "scenario": "Standard Scenario"}, {"value": "0.0", "module": "B3", "scenario": "Standard Scenario"}, {"value": "0.0", "module": "B6", "scenario": "Standard Scenario"}, {"value": "0.0", "module": "B7", "scenario": "Standard Scenario"}, {"value": "0.0", "module": "C1", "scenario": "Standard Scenario"}, {"value": "8.547E-11", "module": "C2", "scenario": "Standard Scenario"}, {"value": "2.77581E-9", "module": "C3", "scenario": "Standard Scenario"}, {"value": "5.35E-12", "module": "C4", "scenario": "Standard Scenario"}, {"value": "-7.1817E-10", "module": "D", "scenario": "Standard Scenario"}, {"name": "referenceToUnitGroupDataSet", "value": {"shortDescription": [{"value": "CTUh", "lang": "en"}], "type": "unit group data set", "refObjectId": "d4c9523e-2d7e-49fd-8469-998f547d3a70", "version": "00.00.003", "uri": "../unitgroups/d4c9523e-2d7e-49fd-8469-998f547d3a70.xml"}}]}}, {"referenceToLCIAMethodDataSet": {"shortDescription": [{"value": "Potential Human exposure efficiency relative to U235 (IRP)", "lang": "en"}, {"value": "Potenzielle Wirkung durch Exposition des Menschen mit U235 (IRP)", "lang": "de"}], "type": "LCIA method data set", "refObjectId": "b5c632be-def3-11e6-bf01-fe55135034f3", "version": "01.00.012", "uri": "../lciamethods/b5c632be-def3-11e6-bf01-fe55135034f3.xml"}, "meanAmount": 0.0, "other": {"anies": [{"value": "0.02443741819674", "module": "A1", "scenario": "Standard Scenario"}, {"value": "9.35676355E-4", "module": "A2", "scenario": "Standard Scenario"}, {"value": "0.01363283790895", "module": "A3", "scenario": "Standard Scenario"}, {"value": "0.03900593246069001", "module": "A1-A3", "scenario": "Standard Scenario"}, {"value": "0.00331155902503", "module": "A4", "scenario": "Standard Scenario"}, {"value": "0.00237577967123", "module": "A5", "scenario": "Standard Scenario"}, {"value": "0.0", "module": "B1", "scenario": "Standard Scenario"}, {"value": "0.0", "module": "B2", "scenario": "Standard Scenario"}, {"value": "0.0", "module": "B3", "scenario": "Standard Scenario"}, {"value": "0.0", "module": "B6", "scenario": "Standard Scenario"}, {"value": "0.0", "module": "B7", "scenario": "Standard Scenario"}, {"value": "0.0", "module": "C1", "scenario": "Standard Scenario"}, {"value": "3.6714832695E-4", "module": "C2", "scenario": "Standard Scenario"}, {"value": "0.00220170632028", "module": "C3", "scenario": "Standard Scenario"}, {"value": "3.019827374E-5", "module": "C4", "scenario": "Standard Scenario"}, {"value": "-0.003131344919", "module": "D", "scenario": "Standard Scenario"}, {"name": "referenceToUnitGroupDataSet", "value": {"shortDescription": [{"value": "kgBq U235-eq.", "lang": "en"}], "type": "unit group data set", "refObjectId": "456b05bf-1415-44a9-9993-02452f554c09", "version": "00.00.003", "uri": "../unitgroups/456b05bf-1415-44a9-9993-02452f554c09.xml"}}]}}, {"referenceToLCIAMethodDataSet": {"shortDescription": [{"value": "Depletion potential of the stratospheric ozone layer (ODP)", "lang": "en"}, {"value": "Abbaupotenzial der stratosphärischen Ozonschicht (ODP)", "lang": "de"}], "type": "LCIA method data set", "refObjectId": "b5c629d6-def3-11e6-bf01-fe55135034f3", "version": "02.00.013", "uri": "../lciamethods/b5c629d6-def3-11e6-bf01-fe55135034f3.xml"}, "meanAmount": 0.0, "other": {"anies": [{"value": "1.917906E-8", "module": "A1", "scenario": "Standard Scenario"}, {"value": "3.26827E-9", "module": "A2", "scenario": "Standard Scenario"}, {"value": "4.46595E-9", "module": "A3", "scenario": "Standard Scenario"}, {"value": "2.6913279999999997E-8", "module": "A1-A3", "scenario": "Standard Scenario"}, {"value": "1.15671E-8", "module": "A4", "scenario": "Standard Scenario"}, {"value": "3.50276E-9", "module": "A5", "scenario": "Standard Scenario"}, {"value": "0.0", "module": "B1", "scenario": "Standard Scenario"}, {"value": "0.0", "module": "B2", "scenario": "Standard Scenario"}, {"value": "0.0", "module": "B3", "scenario": "Standard Scenario"}, {"value": "0.0", "module": "B6", "scenario": "Standard Scenario"}, {"value": "0.0", "module": "B7", "scenario": "Standard Scenario"}, {"value": "0.0", "module": "C1", "scenario": "Standard Scenario"}, {"value": "1.28243E-9", "module": "C2", "scenario": "Standard Scenario"}, {"value": "2.134944E-8", "module": "C3", "scenario": "Standard Scenario"}, {"value": "1.0087E-10", "module": "C4", "scenario": "Standard Scenario"}, {"value": "-6.19647E-8", "module": "D", "scenario": "Standard Scenario"}, {"name": "referenceToUnitGroupDataSet", "value": {"shortDescription": [{"value": "kg CFC-11-eq.", "lang": "en"}], "type": "unit group data set", "refObjectId": "d9e957c9-7309-4474-bf3a-7777df6c4e5b", "version": "25.00.000", "uri": "../unitgroups/d9e957c9-7309-4474-bf3a-7777df6c4e5b.xml"}}]}}, {"referenceToLCIAMethodDataSet": {"shortDescription": [{"value": "Potential incidence of disease due to PM emissions (PM)", "lang": "en"}, {"value": "Potenzielles Auftreten von Krankheiten aufgrund von Feinstaubemissionen (PM)", "lang": "de"}], "type": "LCIA method data set", "refObjectId": "b5c602c6-def3-11e6-bf01-fe55135034f3", "version": "02.00.012", "uri": "../lciamethods/b5c602c6-def3-11e6-bf01-fe55135034f3.xml"}, "meanAmount": 0.0, "other": {"anies": [{"value": "1.855376E-8", "module": "A1", "scenario": "Standard Scenario"}, {"value": "1.33209E-9", "module": "A2", "scenario": "Standard Scenario"}, {"value": "4.1049E-9", "module": "A3", "scenario": "Standard Scenario"}, {"value": "2.3990750000000003E-8", "module": "A1-A3", "scenario": "Standard Scenario"}, {"value": "4.71457E-9", "module": "A4", "scenario": "Standard Scenario"}, {"value": "1.85802E-9", "module": "A5", "scenario": "Standard Scenario"}, {"value": "0.0", "module": "B1", "scenario": "Standard Scenario"}, {"value": "0.0", "module": "B2", "scenario": "Standard Scenario"}, {"value": "0.0", "module": "B3", "scenario": "Standard Scenario"}, {"value": "0.0", "module": "B6", "scenario": "Standard Scenario"}, {"value": "0.0", "module": "B7", "scenario": "Standard Scenario"}, {"value": "0.0", "module": "C1", "scenario": "Standard Scenario"}, {"value": "5.227E-10", "module": "C2", "scenario": "Standard Scenario"}, {"value": "2.50058E-9", "module": "C3", "scenario": "Standard Scenario"}, {"value": "5.351E-11", "module": "C4", "scenario": "Standard Scenario"}, {"value": "-2.29177E-9", "module": "D", "scenario": "Standard Scenario"}, {"name": "referenceToUnitGroupDataSet", "value": {"shortDescription": [{"value": "Disease incidence", "lang": "en"}], "type": "unit group data set", "refObjectId": "3883559b-648f-4afc-8ba2-0bd24f3affa3", "version": "00.00.003", "uri": "../unitgroups/3883559b-648f-4afc-8ba2-0bd24f3affa3.xml"}}]}}, {"referenceToLCIAMethodDataSet": {"shortDescription": [{"value": "Photochemical Ozone Creation Potential (POCP)", "lang": "en"}, {"value": "Bildungspotenzial für troposphärisches Ozon (POCP)", "lang": "de"}], "type": "LCIA method data set", "refObjectId": "b5c610fe-def3-11e6-bf01-fe55135034f3", "version": "02.00.015", "uri": "../lciamethods/b5c610fe-def3-11e6-bf01-fe55135034f3.xml"}, "meanAmount": 0.0, "other": {"anies": [{"value": "0.00260281941677", "module": "A1", "scenario": "Standard Scenario"}, {"value": "9.525395133E-5", "module": "A2", "scenario": "Standard Scenario"}, {"value": "2.4529622114E-4", "module": "A3", "scenario": "Standard Scenario"}, {"value": "0.00294336958924", "module": "A1-A3", "scenario": "Standard Scenario"}, {"value": "3.371241354E-4", "module": "A4", "scenario": "Standard Scenario"}, {"value": "2.0276502605E-4", "module": "A5", "scenario": "Standard Scenario"}, {"value": "0.0", "module": "B1", "scenario": "Standard Scenario"}, {"value": "0.0", "module": "B2", "scenario": "Standard Scenario"}, {"value": "0.0", "module": "B3", "scenario": "Standard Scenario"}, {"value": "0.0", "module": "B6", "scenario": "Standard Scenario"}, {"value": "0.0", "module": "B7", "scenario": "Standard Scenario"}, {"value": "0.0", "module": "C1", "scenario": "Standard Scenario"}, {"value": "3.737652307E-5", "module": "C2", "scenario": "Standard Scenario"}, {"value": "2.55378375E-4", "module": "C3", "scenario": "Standard Scenario"}, {"value": "3.99773481E-6", "module": "C4", "scenario": "Standard Scenario"}, {"value": "-5.286172178E-4", "module": "D", "scenario": "Standard Scenario"}, {"name": "referenceToUnitGroupDataSet", "value": {"shortDescription": [{"value": "kg NMVOC-eq.", "lang": "en"}], "type": "unit group data set", "refObjectId": "d27c25f8-fbc1-44c6-b47b-4adbae4199c6", "version": "00.00.003", "uri": "../unitgroups/d27c25f8-fbc1-44c6-b47b-4adbae4199c6.xml"}}]}}, {"referenceToLCIAMethodDataSet": {"shortDescription": [{"value": "Potential Soil quality index (SQP)", "lang": "en"}, {"value": "Potenzieller Bodenqualitätsindex (SQP)", "lang": "de"}], "type": "LCIA method data set", "refObjectId": "b2ad6890-c78d-11e6-9d9d-cec0c932ce01", "version": "01.00.011", "uri": "../lciamethods/b2ad6890-c78d-11e6-9d9d-cec0c932ce01.xml"}, "meanAmount": 0.0, "other": {"anies": [{"value": "1.32501661128813", "module": "A1", "scenario": "Standard Scenario"}, {"value": "0.19367218142864", "module": "A2", "scenario": "Standard Scenario"}, {"value": "4.39335864063452", "module": "A3", "scenario": "Standard Scenario"}, {"value": "5.91204743335129", "module": "A1-A3", "scenario": "Standard Scenario"}, {"value": "0.6854473311009", "module": "A4", "scenario": "Standard Scenario"}, {"value": "0.35925613148188", "module": "A5", "scenario": "Standard Scenario"}, {"value": "0.0", "module": "B1", "scenario": "Standard Scenario"}, {"value": "0.0", "module": "B2", "scenario": "Standard Scenario"}, {"value": "0.0", "module": "B3", "scenario": "Standard Scenario"}, {"value": "0.0", "module": "B6", "scenario": "Standard Scenario"}, {"value": "0.0", "module": "B7", "scenario": "Standard Scenario"}, {"value": "0.0", "module": "C1", "scenario": "Standard Scenario"}, {"value": "0.07599467167061", "module": "C2", "scenario": "Standard Scenario"}, {"value": "0.19165731125805", "module": "C3", "scenario": "Standard Scenario"}, {"value": "0.01824535416619", "module": "C4", "scenario": "Standard Scenario"}, {"value": "-3.44451341201975", "module": "D", "scenario": "Standard Scenario"}, {"name": "referenceToUnitGroupDataSet", "value": {"shortDescription": [{"value": "dimensionless", "lang": "en"}], "type": "unit group data set", "refObjectId": "f130951c-e67f-4f7f-8dd4-665de3974e18", "version": "00.00.004", "uri": "../unitgroups/f130951c-e67f-4f7f-8dd4-665de3974e18.xml"}}]}}, {"referenceToLCIAMethodDataSet": {"shortDescription": [{"value": "Water (user) deprivation potential (WDP)", "lang": "en"}, {"value": "Wasser-Entzugspotenzial (Benutzer) (WDP)", "lang": "de"}], "type": "LCIA method data set", "refObjectId": "b2ad66ce-c78d-11e6-9d9d-cec0c932ce01", "version": "03.00.015", "uri": "../lciamethods/b2ad66ce-c78d-11e6-9d9d-cec0c932ce01.xml"}, "meanAmount": 0.0, "other": {"anies": [{"value": "0.71216733405775", "module": "A1", "scenario": "Standard Scenario"}, {"value": "7.9896925902E-4", "module": "A2", "scenario": "Standard Scenario"}, {"value": "0.05221571033272", "module": "A3", "scenario": "Standard Scenario"}, {"value": "0.76518201364949", "module": "A1-A3", "scenario": "Standard Scenario"}, {"value": "0.0028277233322", "module": "A4", "scenario": "Standard Scenario"}, {"value": "0.04050825589505", "module": "A5", "scenario": "Standard Scenario"}, {"value": "0.0", "module": "B1", "scenario": "Standard Scenario"}, {"value": "0.0", "module": "B2", "scenario": "Standard Scenario"}, {"value": "0.0", "module": "B3", "scenario": "Standard Scenario"}, {"value": "0.0", "module": "B6", "scenario": "Standard Scenario"}, {"value": "0.0", "module": "B7", "scenario": "Standard Scenario"}, {"value": "0.0", "module": "C1", "scenario": "Standard Scenario"}, {"value": "3.1350608056E-4", "module": "C2", "scenario": "Standard Scenario"}, {"value": "0.03554258401798", "module": "C3", "scenario": "Standard Scenario"}, {"value": "3.3058191719E-4", "module": "C4", "scenario": "Standard Scenario"}, {"value": "-0.05168620374264", "module": "D", "scenario": "Standard Scenario"}, {"name": "referenceToUnitGroupDataSet", "value": {"shortDescription": [{"value": "m3 world eq. deprived", "lang": "en"}], "type": "unit group data set", "refObjectId": "6ae2df01-888e-46c8-b17d-49fa3869b476", "version": "00.00.003", "uri": "../unitgroups/6ae2df01-888e-46c8-b17d-49fa3869b476.xml"}}]}}]}, "otherAttributes": {"{http://www.indata.network/EPD/2019}epd-version": "1.2"}, "version": "1.1"}