{"processInformation": {"dataSetInformation": {"UUID": "c75af9d3-f5f1-4712-a82c-d66bf8282969", "name": {"baseName": [{"value": "LA GARD 700", "lang": "en"}, {"value": "LA GARD 700", "lang": "de"}], "functionalUnitFlowProperties": [{"lang": "en"}]}, "classificationInformation": {"classification": [{"class": [{"value": "Komponenten von Fenstern und Vorhangfassaden", "level": 0, "classId": "7"}, {"value": "Beschläge", "level": 1, "classId": "7.4"}, {"value": "Befestigungen", "level": 2, "classId": "7.4.06"}], "name": "OEKOBAU.DAT"}, {"class": [{"value": "02 Building products", "level": 0}, {"value": "Doors, windows, shutters, and related products", "level": 1}, {"value": "Electronic and physical Access Control Systems", "level": 2}], "name": "IBUCategories"}]}, "generalComment": [{"value": "LA GARD has been an industry leader in the safe lock sector for nearly half of a century.\n\nThe LA GARD 700 Series embodies the original tried-and-true features\nand long legacy of LA GARD high-security function along with advanced\ntechnological features.\nThe series offers a range of features and options to fit almost any\nsafe lock need.\n\nSecurity – the electronic safe locks are designed to support the ever-changing needs of todays world\nEfficiency – lower total cost of ownership, fewer battery changes, ease of use, simplified inventory management\nConfidence – from a name you know and trust \nUser Experience – unified software platform, feature-rich OLED display, simplified user-prompts \nExcellence – quality commitment backed by 2 year warranty; extended warranty\navailable, world-class support, modern dormakaba design aesthetic\nDisplay – OLED keypad featuring on-screen promptsFor placing the LA GARD 700 Series electronic safe lock on the market in the European Union/European Free Trade Association (EU/EFTA) (with the exception of Switzerland) the following legal provisions apply:\n\nVdS 2344:2014-07\nVdS 2396:2014-07\n\nUL 2058:2005-06\n\nDIN EN1300:2019-05\n\nRestriction of Hazardous Substances (RoHS)", "lang": "en"}, {"value": "LA GARD ist seit fast einem halben Jahrhundert führend auf dem Gebiet der Tresorschlösser. Die LA GARD 700er Serie verkörpert die ursprünglichen, bewährten Merkmale und das lange Erbe der LA GARD Hochsicherheitsfunktionen zusammen mit fortschrittlichen technologischen Merkmalen. Die Serie bietet eine Reihe von Merkmalen und Optionen, die nahezu alle Anforderungen an Tresorschlösser erfüllen.\n\nSicherheit - die elektronischen Tresorschlösser sind so konzipiert, dass sie den sich ständig ändernden Anforderungen der heutigen Welt gerecht werden Effizienz - geringere Gesamtbetriebskosten, weniger Batteriewechsel, einfache Bedienung, vereinfachte Bestandsverwaltung Vertrauen - von einem Namen, den Sie kennen und dem Sie vertrauen Benutzerfreundlichkeit - einheitliche Softwareplattform, funktionsreiches OLED-Display, vereinfachte Benutzerführung Exzellenz - Qualitätsverpflichtung durch 2 Jahre Garantie gesichert; Garantieverlängerung verfügbar, erstklassiger Support, modernes dormakaba Design Ästhetik Anzeige - OLED-Tastatur mit BildschirmanweisungenFür das Inverkehrbringen des elektronischen Tresorschlosses der LA GARD 700 Serie in der Europäischen Union/Europäischen Freihandelszone (EU/EFTA) (mit Ausnahme der Schweiz) gelten die folgenden gesetzlichen Bestimmungen:\n\nVdS 2344:2014-07 VdS 2396:2014-07 UL 2058:2005-06 DIN EN1300:2019-05 Restriction of Hazardous Substances (RoHS)", "lang": "de"}], "other": {"anies": [{"scenario": [{"description": [{"value": "EU-28 electricity grid mix", "lang": "en"}, {"value": "Stromnetzmix der EU-28", "lang": "de"}], "name": "S1", "default": true}, {"description": [{"value": "US electricity grid mix", "lang": "en"}, {"value": "US-Stromnetz-Mix", "lang": "de"}], "name": "S2"}]}]}}, "quantitativeReference": {"referenceToReferenceFlow": [0]}, "time": {"referenceYear": 2022, "dataSetValidUntil": 2027, "other": {"anies": [{"name": "publicationDateOfEPD", "value": 1644883200000}]}}, "geography": {"locationOfOperationSupplyOrProduction": {"location": "MX"}}, "technology": {"technologyDescriptionAndIncludedProcesses": [{"value": "The LA GARD 700 Series safe lock is the ideal for commercial industries, vault storage, government and residential/personal applications. \nTechnical data: \nFollowing technical specification applies for LA GARD 700 Series: \nDeclared unit: \nThe declared unit is 1 piece of the product: 0.606 kg", "lang": "en"}, {"value": "Das LA GARD Tresorschloss der Serie 700 ist ideal für die gewerbliche Industrie, Tresorräume, Behörden und private Anwendungen. \nTechnische Daten: \nDie folgenden technischen Daten gelten für die LA GARD 700 Serie: \nDeklarierte Einheit: \nDie angegebene Einheit ist 1 Stück des Produkts: 0,606 kg", "lang": "de"}], "technologicalApplicability": [{"value": "The LA GARD 700 Series is the ideal for commercial industries, vault storage, government and residential/personal applications like:\n\nResidential\n\nCommerial retail\n\nQuick serve restaurants\n\nATM and currency exchange\n\nPharmacies\n\nLaw enforcement facilities\n\nValut storage\n\nCash recyclers\n\nMilitary institutionsWith five models (Models 701-705) to choose from, the series offers a range of features and options to fit almost any safe lock need. Following models are available:\n\nModel 701 – basic offering\n\nModel 702 – multi-user lock standard keypad\n\nModel 703 – multi-user, 2-lock system, display\n\nModel 704 – multi-user, 5-lock system, display\n\nModel 705 – multi-user, 5-lock system, displa", "lang": "en"}, {"value": "Die LA GARD 700 Serie ist ideal für gewerbliche Anwendungen, Tresorräume, Behörden und private Anwendungen, wie z.B.: Wohngebäude Einzelhandel Schnellrestaurants Geldautomaten und Geldwechsel Apotheken Strafverfolgungsbehörden Wertaufbewahrung Bargeldverwertung Militärische EinrichtungenMit fünf Modellen (Modelle 701-705) zur Auswahl bietet die Serie eine Reihe von Funktionen und Optionen, die nahezu alle Anforderungen an ein Tresorschloss erfüllen. Folgende Modelle sind erhältlich: Modell 701 - Basisangebot Modell 702 - Mehrbenutzerschloss mit Standardtastatur Modell 703 - Mehrbenutzer, 2-Schloss-System, Display Modell 704 - Mehrbenutzer, 5-Schloss-System, Display Modell 705 - Mehrbenutzer, 5-Schloss-System, Displa", "lang": "de"}]}}, "modellingAndValidation": {"LCIMethodAndAllocation": {"typeOfDataSet": "EPD", "referenceToLCAMethodDetails": [{"shortDescription": [{"value": "Electronic and physical Access Control Systems.pdf", "lang": "en"}], "type": "source data set", "refObjectId": "30922b52-134f-4dbf-bc65-ef2973f1b50f"}], "other": {"anies": [{"name": "subType", "value": "specific dataset"}]}}, "dataSourcesTreatmentAndRepresentativeness": {"referenceToDataSource": [{"shortDescription": [{"value": "GaBi Database (all versions)", "lang": "en"}], "type": "source data set", "refObjectId": "28d74cc0-db8b-4d7e-bc44-5f6d56ce0c4a"}, {"shortDescription": [{"value": "GaBi Database Edition 2020, CUP 2020.02", "lang": "en"}], "type": "source data set", "refObjectId": "4b368ada-d799-4afc-9d41-f371f2b23781"}], "useAdviceForDataSet": [{"value": "Scope: \nThis declaration is a specific product declaration for the LA GARD 700 series electronic safe lock.\nThe underlying life cycle assessment is based on the entire life cycle of this specific LA GARD 700 Series electronic safe lock manufactured by dormakaba. The various technical features are outlined in chapter 2. The products are manufactured at the dormakaba production facility in Nogales (Mexico). The year of data collection is 2021. The declared product is not including the batteries and energy supply modules \nSystem boundary: \nThe type of EPD is: cradle to gate with options, modules C1–C4, and module D (A1–A3 + C + D and additional modules: A4 + A5 + B6)\n\nProduction - Module A1-A3\nThe product stage includes:\n— A1, raw material extraction, processing and mechanical treatments, processing of secondary material input (e.g. recycling processes),\n— A2, transport to the manufacturer,\n— A3, manufacturing and assembly including provision of all materials, products and energy, as well as waste processing up to the end-of waste state.\n\nConstruction stage - Modules A4-A5\nThe construction process stage includes:\n— A4, transport to the building site;\n— A5, installation into the building; including provision of all materials, products and energy, as well as waste processing up to the end-of-waste state or disposal of final residues during the construction process stage.\n\nMaintenance – Module B2\nThis module includes the production and the end of life of the batteries. The potential use of batteries is declared in module B2.\n\nUse stage - Module B6\nThe use stage related to the operation of the building includes:\n— B6, operational energy use\nThe potential use of electricity from the grid is declared in module B6.\n\nEnd-of-life stage– Modules C1-C4 and D\nThe end-of-life stage includes:\n— C1, de-construction, demolition:\n— C2, transport to waste processing;\n— C3, waste processing for reuse, recovery and/or recycling;\n— C4, disposal; including provision and all transport, provision of all materials, products and related energy and water use.\n\nModule D (Benefits and loads beyond the system boundary) includes:\n— D, recycling potentials, expressed as net impacts and benefits.", "lang": "en"}, {"value": "Gültigkeitsbereich: \nDiese Deklaration ist eine spezifische Produktdeklaration für das elektronische Tresorschloss der Serie LA GARD 700. Die zugrunde liegende Ökobilanz basiert auf dem gesamten Lebenszyklus dieses spezifischen elektronischen Tresorschlosses der Serie LA GARD 700 von dormakaba. Die verschiedenen technischen Merkmale werden in Kapitel 2 beschrieben. Die Produkte werden in der dormakaba Produktionsstätte in Nogales (Mexiko) hergestellt. Das Jahr der Datenerhebung ist 2021. Das angegebene Produkt enthält nicht die Batterien und Energieversorgungsmodule \nSystemgrenze: \nDie Art der EPD ist: Cradle to Gate mit Optionen, Modulen C1-C4 und Modul D (A1-A3 + C + D und zusätzliche Module: A4 + A5 + B6) Produktion - Modul A1-A3 Die Produktphase umfasst: - A1, Rohstoffgewinnung, Verarbeitung und mechanische Behandlungen, Verarbeitung von Sekundärmaterialinput (z.B. Recyclingprozesse), - A2, Transport zum Hersteller, - A3, Herstellung und Montage einschließlich Bereitstellung aller Materialien, Produkte und Energie sowie Abfallverarbeitung bis zum End-of-Waste-Zustand.\n\nBauphase - Module A4-A5 Die Bauphase umfasst: - A4, Transport zur Baustelle; - A5, Einbau in das Gebäude; einschließlich der Bereitstellung aller Materialien, Produkte und Energie sowie der Abfallverarbeitung bis zum Ende des Abfallzustands oder der Beseitigung der endgültigen Rückstände während der Bauphase. Wartung - Modul B2 Dieses Modul umfasst die Produktion und das Ende der Lebensdauer der Batterien. Die potenzielle Nutzung der Batterien wird in Modul B2 angegeben. Nutzungsphase - Modul B6 Die Nutzungsphase im Zusammenhang mit dem Betrieb des Gebäudes umfasst: - B6, Betriebliche Energienutzung Die potenzielle Nutzung von Strom aus dem Netz wird in Modul B6 angegeben.\n\nEnd-of-Life-Phase - Module C1-C4 und D Die End-of-Life-Phase umfasst: - C1, Rückbau, Abriss; - C2, Transport zur Abfallverarbeitung; - C3, Abfallverarbeitung zur Wiederverwendung, Wiederverwertung und/oder zum Recycling; - C4, Entsorgung; einschließlich Bereitstellung und sämtlicher Transporte, Bereitstellung aller Materialien, Produkte und des damit verbundenen Energie- und Wasserverbrauchs. Modul D (Nutzen und Lasten jenseits der Systemgrenze) umfasst: - D, Recyclingpotenziale, ausgedrückt als Nettoauswirkungen und Nutzen.", "lang": "de"}], "other": {"anies": [{"name": "referenceToOriginalEPD", "value": {"shortDescription": {"value": "LA GARD 700 .pdf", "defaultValue": "LA GARD 700 .pdf", "lstrings": [{"lang": "en", "value": "LA GARD 700 .pdf"}]}, "type": "source data set", "uuid": {"uuid": "3b934aa3-3b72-44cb-869a-ce81cb6f8ce5"}, "refObjectId": "3b934aa3-3b72-44cb-869a-ce81cb6f8ce5", "resourceURLs": ["https://oekobaudat.de/OEKOBAU.DAT/resource/sources/3b934aa3-3b72-44cb-869a-ce81cb6f8ce5/LA_GARD_700_22777.pdf?version=00.06.000"]}}]}}, "validation": {"review": [{"referenceToNameOfReviewerAndInstitution": [{"shortDescription": [{"value": "Institut Bauen und Umwelt e. V.", "lang": "en"}], "type": "contact data set", "refObjectId": "d111dbec-b024-4be5-86c5-752d6eb2cf95", "uri": "../contacts/d111dbec-b024-4be5-86c5-752d6eb2cf95.xml"}], "type": "Accredited third party review"}]}, "complianceDeclarations": {"compliance": [{"referenceToComplianceSystem": {"shortDescription": [{"value": "DIN EN 15804+A2", "lang": "en"}], "type": "source data set", "refObjectId": "c0016b33-8cf7-415c-ac6e-deba0d21440d", "uri": "../sources/c0016b33-8cf7-415c-ac6e-deba0d21440d.xml"}}, {"referenceToComplianceSystem": {"shortDescription": [{"value": "ISO 14025", "lang": "en"}], "type": "source data set", "refObjectId": "4f2eb655-6e44-4874-a95a-e28f5442cd4d", "uri": "../sources/4f2eb655-6e44-4874-a95a-e28f5442cd4d.xml"}}]}}, "administrativeInformation": {"commissionerAndGoal": {"referenceToCommissioner": [{"shortDescription": [{"value": "dormakaba International Holding GmbH", "lang": "en"}], "type": "contact data set", "refObjectId": "33313944-7b37-498a-b458-25a295c1017d", "uri": "../contacts/33313944-7b37-498a-b458-25a295c1017d.xml"}]}, "dataGenerator": {"referenceToPersonOrEntityGeneratingTheDataSet": [{"shortDescription": [{"value": "Sphera Solutions GmbH", "lang": "en"}], "type": "contact data set", "refObjectId": "623edf96-39d1-4e6f-9892-674c7228546b", "uri": "../contacts/623edf96-39d1-4e6f-9892-674c7228546b.xml"}]}, "dataEntryBy": {"timeStamp": 1644883200000, "referenceToDataSetFormat": [{"shortDescription": [{"value": "ILCD Format", "lang": "en"}], "type": "source data set", "refObjectId": "a97a0155-0234-4b87-b4ce-a45da52f2a40", "uri": "../sources/a97a0155-0234-4b87-b4ce-a45da52f2a40.xml"}, {"shortDescription": [{"value": "EPD-Datenformaterweiterungen v1.2", "lang": "de"}, {"value": "EPD Data Format Extensions v1.2", "lang": "en"}], "type": "source data set", "refObjectId": "a29449fd-aa2f-4de8-b5d7-4b06b43c6fde", "uri": "../sources/a29449fd-aa2f-4de8-b5d7-4b06b43c6fde.xml"}]}, "publicationAndOwnership": {"dataSetVersion": "00.08.000", "referenceToRegistrationAuthority": {"shortDescription": [{"value": "Institut Bauen und Umwelt e. V.", "lang": "en"}], "type": "contact data set", "refObjectId": "d111dbec-b024-4be5-86c5-752d6eb2cf95", "uri": "../contacts/d111dbec-b024-4be5-86c5-752d6eb2cf95.xml"}, "registrationNumber": "EPD-DOR-20210247-CBA3-EN", "referenceToOwnershipOfDataSet": {"shortDescription": [{"value": "dormakaba International Holding GmbH", "lang": "en"}], "type": "contact data set", "refObjectId": "33313944-7b37-498a-b458-25a295c1017d", "uri": "../contacts/33313944-7b37-498a-b458-25a295c1017d.xml"}, "copyright": true, "licenseType": "Free of charge for all users and uses", "accessRestrictions": [{"value": "None", "lang": "en"}], "other": {"anies": [{"name": "referenceToPublisher", "value": {"shortDescription": [{"value": "Institut Bauen und Umwelt e. V.", "lang": "en"}], "type": "contact data set", "refObjectId": "d111dbec-b024-4be5-86c5-752d6eb2cf95", "uri": "../contacts/d111dbec-b024-4be5-86c5-752d6eb2cf95.xml"}}]}}}, "exchanges": {"exchange": [{"dataSetInternalID": 0, "referenceToFlowDataSet": {"shortDescription": [{"value": "LA GARD 700 (LA GARD 700)", "lang": "en"}], "type": "flow data set", "refObjectId": "4734be16-4a68-c731-fcaa-d29c1ad45105", "uri": "../flows/4734be16-4a68-c731-fcaa-d29c1ad45105.xml"}, "meanAmount": 1.0, "referencesToDataSource": {}, "referenceFlow": true, "resolvedFlowVersion": "00.05.000", "resultingflowAmount": 1.0, "flowProperties": [{"name": [{"lang": "de", "value": "Anzahl"}, {"lang": "en", "value": "Number of pieces"}], "uuid": "01846770-4cfe-4a25-8ad9-919d8d378345", "referenceFlowProperty": true, "meanValue": 1.0, "referenceUnit": "pcs.", "unitGroupUUID": "934110e3-baf4-49e9-992c-3d8109a6aafb"}, {"name": [{"lang": "en", "value": "Weight"}], "uuid": "93a60a56-a3c8-11da-a746-0800200b9a66", "meanValue": 0.606}], "materialProperties": [{"name": "weight per piece", "value": "0.606", "unit": "kg"}], "typeOfFlow": "Product flow", "classification": {"classHierarchy": "Sonstige /  / ", "name": "OEKOBAU.DAT"}}, {"dataSetInternalID": 1, "referenceToFlowDataSet": {"shortDescription": [{"value": "Renewable primary energy as energy carrier (PERE)", "lang": "en"}, {"value": "Erneuerbare Primärenergie als Energieträger (PERE)", "lang": "de"}], "type": "flow data set", "refObjectId": "20f32be5-0398-4288-9b6d-accddd195317", "uri": "../flows/20f32be5-0398-4288-9b6d-accddd195317.xml"}, "exchange direction": "INPUT", "other": {"anies": [{"name": "referenceToUnitGroupDataSet", "value": {"shortDescription": [{"value": "MJ", "lang": "en"}], "type": "unit group data set", "refObjectId": "93a60a57-a3c8-11da-a746-0800200c9a66", "uri": "../unitgroups/93a60a57-a3c8-11da-a746-0800200c9a66.xml"}}, {"value": "30.32937", "module": "A1-A3"}, {"value": "0.0348", "module": "A4"}, {"value": "0.152", "module": "A5"}, {"value": "0.777", "module": "B2"}, {"value": "0.119", "module": "B6", "scenario": "S1"}, {"value": "0.0621", "module": "B6", "scenario": "S2"}, {"value": "0", "module": "C1"}, {"value": "0.000113", "module": "C2"}, {"value": "0.0563", "module": "C3"}, {"value": "0.000513", "module": "C4"}, {"value": "-5.3", "module": "D"}]}, "resolvedFlowVersion": "38.00.000", "flowProperties": [], "typeOfFlow": "Other flow", "classification": {"classHierarchy": "Quantities", "name": "GaBiCategories"}}, {"dataSetInternalID": 2, "referenceToFlowDataSet": {"shortDescription": [{"value": "Renewable primary energy resources as material utilization (PERM)", "lang": "en"}, {"value": "Erneuerbare Primärenergie zur stofflichen Nutzung (PERM)", "lang": "de"}], "type": "flow data set", "refObjectId": "fb3ec0de-548d-4508-aea5-00b73bf6f702", "uri": "../flows/fb3ec0de-548d-4508-aea5-00b73bf6f702.xml"}, "exchange direction": "INPUT", "other": {"anies": [{"name": "referenceToUnitGroupDataSet", "value": {"shortDescription": [{"value": "MJ", "lang": "en"}], "type": "unit group data set", "refObjectId": "93a60a57-a3c8-11da-a746-0800200c9a66", "uri": "../unitgroups/93a60a57-a3c8-11da-a746-0800200c9a66.xml"}}, {"value": "0.1774", "module": "A1-A3"}, {"value": "0", "module": "A4"}, {"value": "-0.151", "module": "A5"}, {"value": "0", "module": "B2"}, {"value": "0", "module": "B6", "scenario": "S1"}, {"value": "0", "module": "B6", "scenario": "S2"}, {"value": "0", "module": "C1"}, {"value": "0", "module": "C2"}, {"value": "-0.0264", "module": "C3"}, {"value": "0", "module": "C4"}, {"value": "0", "module": "D"}]}, "resolvedFlowVersion": "38.00.000", "flowProperties": [], "typeOfFlow": "Other flow", "classification": {"classHierarchy": "Quantities", "name": "GaBiCategories"}}, {"dataSetInternalID": 3, "referenceToFlowDataSet": {"shortDescription": [{"value": "Total use of renewable primary energy resources (PERT)", "lang": "en"}, {"value": "Total erneuerbare Primärenergie (PERT)", "lang": "de"}], "type": "flow data set", "refObjectId": "53f97275-fa8a-4cdd-9024-65936002acd0", "uri": "../flows/53f97275-fa8a-4cdd-9024-65936002acd0.xml"}, "exchange direction": "INPUT", "other": {"anies": [{"name": "referenceToUnitGroupDataSet", "value": {"shortDescription": [{"value": "MJ", "lang": "en"}], "type": "unit group data set", "refObjectId": "93a60a57-a3c8-11da-a746-0800200c9a66", "uri": "../unitgroups/93a60a57-a3c8-11da-a746-0800200c9a66.xml"}}, {"value": "30.58037", "module": "A1-A3"}, {"value": "0.0348", "module": "A4"}, {"value": "0.00102", "module": "A5"}, {"value": "0.777", "module": "B2"}, {"value": "0.119", "module": "B6", "scenario": "S1"}, {"value": "0.0621", "module": "B6", "scenario": "S2"}, {"value": "0", "module": "C1"}, {"value": "0.000113", "module": "C2"}, {"value": "0.0299", "module": "C3"}, {"value": "0.000513", "module": "C4"}, {"value": "-5.3", "module": "D"}]}, "resolvedFlowVersion": "38.00.000", "flowProperties": [], "typeOfFlow": "Other flow", "classification": {"classHierarchy": "Quantities / Environmental quantities / EPD EN 15804 / LCI indicators", "name": "GaBiCategories"}}, {"dataSetInternalID": 4, "referenceToFlowDataSet": {"shortDescription": [{"value": "Non renewable primary energy as energy carrier (PENRE)", "lang": "en"}, {"value": "Nicht-erneuerbare Primärenergie als Energieträger (PENRE)", "lang": "de"}], "type": "flow data set", "refObjectId": "ac857178-2b45-46ec-892a-a9a4332f0372", "uri": "../flows/ac857178-2b45-46ec-892a-a9a4332f0372.xml"}, "exchange direction": "INPUT", "other": {"anies": [{"name": "referenceToUnitGroupDataSet", "value": {"shortDescription": [{"value": "MJ", "lang": "en"}], "type": "unit group data set", "refObjectId": "93a60a57-a3c8-11da-a746-0800200c9a66", "uri": "../unitgroups/93a60a57-a3c8-11da-a746-0800200c9a66.xml"}}, {"value": "210.52", "module": "A1-A3"}, {"value": "14.4", "module": "A4"}, {"value": "0.00564", "module": "A5"}, {"value": "3.86", "module": "B2"}, {"value": "0.268", "module": "B6", "scenario": "S1"}, {"value": "0.342", "module": "B6", "scenario": "S2"}, {"value": "0", "module": "C1"}, {"value": "0.036", "module": "C2"}, {"value": "3.54", "module": "C3"}, {"value": "0.00392", "module": "C4"}, {"value": "-41.1", "module": "D"}]}, "resolvedFlowVersion": "38.00.000", "flowProperties": [], "typeOfFlow": "Other flow", "classification": {"classHierarchy": "Quantities", "name": "GaBiCategories"}}, {"dataSetInternalID": 5, "referenceToFlowDataSet": {"shortDescription": [{"value": "Non renewable primary energy as material utilization (PENRM)", "lang": "en"}, {"value": "Nicht-erneuerbare Primärenergie zur stofflichen Nutzung (PENRM)", "lang": "de"}], "type": "flow data set", "refObjectId": "1421caa0-679d-4bf4-b282-0eb850ccae27", "uri": "../flows/1421caa0-679d-4bf4-b282-0eb850ccae27.xml"}, "exchange direction": "INPUT", "other": {"anies": [{"name": "referenceToUnitGroupDataSet", "value": {"shortDescription": [{"value": "MJ", "lang": "en"}], "type": "unit group data set", "refObjectId": "93a60a57-a3c8-11da-a746-0800200c9a66", "uri": "../unitgroups/93a60a57-a3c8-11da-a746-0800200c9a66.xml"}}, {"value": "3.43", "module": "A1-A3"}, {"value": "0", "module": "A4"}, {"value": "0", "module": "A5"}, {"value": "0", "module": "B2"}, {"value": "0", "module": "B6", "scenario": "S1"}, {"value": "0", "module": "B6", "scenario": "S2"}, {"value": "0", "module": "C1"}, {"value": "0", "module": "C2"}, {"value": "-3.43", "module": "C3"}, {"value": "0", "module": "C4"}, {"value": "0", "module": "D"}]}, "resolvedFlowVersion": "38.00.000", "flowProperties": [], "typeOfFlow": "Other flow", "classification": {"classHierarchy": "Quantities", "name": "GaBiCategories"}}, {"dataSetInternalID": 6, "referenceToFlowDataSet": {"shortDescription": [{"value": "Total use of non renewable primary energy resources (PENRT)", "lang": "en"}, {"value": "Total nicht erneuerbare Primärenergie (PENRT)", "lang": "de"}], "type": "flow data set", "refObjectId": "06159210-646b-4c8d-8583-da9b3b95a6c1", "uri": "../flows/06159210-646b-4c8d-8583-da9b3b95a6c1.xml"}, "exchange direction": "INPUT", "other": {"anies": [{"name": "referenceToUnitGroupDataSet", "value": {"shortDescription": [{"value": "MJ", "lang": "en"}], "type": "unit group data set", "refObjectId": "93a60a57-a3c8-11da-a746-0800200c9a66", "uri": "../unitgroups/93a60a57-a3c8-11da-a746-0800200c9a66.xml"}}, {"value": "213.52", "module": "A1-A3"}, {"value": "14.4", "module": "A4"}, {"value": "0.00564", "module": "A5"}, {"value": "3.86", "module": "B2"}, {"value": "0.268", "module": "B6", "scenario": "S1"}, {"value": "0.342", "module": "B6", "scenario": "S2"}, {"value": "0", "module": "C1"}, {"value": "0.036", "module": "C2"}, {"value": "0.115", "module": "C3"}, {"value": "0.00392", "module": "C4"}, {"value": "-41.1", "module": "D"}]}, "resolvedFlowVersion": "38.00.000", "flowProperties": [], "typeOfFlow": "Other flow", "classification": {"classHierarchy": "Quantities / Environmental quantities / EPD EN 15804 / LCI indicators", "name": "GaBiCategories"}}, {"dataSetInternalID": 7, "referenceToFlowDataSet": {"shortDescription": [{"value": "Use of secondary material (SM)", "lang": "en"}, {"value": "Einsatz von Sekundärstoffen (SM)", "lang": "de"}], "type": "flow data set", "refObjectId": "c6a1f35f-2d09-4f54-8dfb-97e502e1ce92", "uri": "../flows/c6a1f35f-2d09-4f54-8dfb-97e502e1ce92.xml"}, "exchange direction": "INPUT", "other": {"anies": [{"name": "referenceToUnitGroupDataSet", "value": {"shortDescription": [{"value": "kg", "lang": "en"}], "type": "unit group data set", "refObjectId": "ad38d542-3fe9-439d-9b95-2f5f7752acaf", "uri": "../unitgroups/ad38d542-3fe9-439d-9b95-2f5f7752acaf.xml"}}, {"value": "0.0317", "module": "A1-A3"}, {"value": "0", "module": "A4"}, {"value": "0", "module": "A5"}, {"value": "0", "module": "B2"}, {"value": "0", "module": "B6", "scenario": "S1"}, {"value": "0", "module": "B6", "scenario": "S2"}, {"value": "0", "module": "C1"}, {"value": "0", "module": "C2"}, {"value": "0", "module": "C3"}, {"value": "0", "module": "C4"}, {"value": "0", "module": "D"}]}, "resolvedFlowVersion": "38.00.000", "flowProperties": [], "typeOfFlow": "Other flow", "classification": {"classHierarchy": "Quantities / Environmental quantities / EPD EN 15804 / LCI indicators", "name": "GaBiCategories"}}, {"dataSetInternalID": 8, "referenceToFlowDataSet": {"shortDescription": [{"value": "Use of renewable secondary fuels (RSF)", "lang": "en"}, {"value": "Erneuerbare Sekundärbrennstoffe (RSF)", "lang": "de"}], "type": "flow data set", "refObjectId": "64333088-a55f-4aa2-9a31-c10b07816787", "uri": "../flows/64333088-a55f-4aa2-9a31-c10b07816787.xml"}, "exchange direction": "INPUT", "other": {"anies": [{"name": "referenceToUnitGroupDataSet", "value": {"shortDescription": [{"value": "MJ", "lang": "en"}], "type": "unit group data set", "refObjectId": "93a60a57-a3c8-11da-a746-0800200c9a66", "uri": "../unitgroups/93a60a57-a3c8-11da-a746-0800200c9a66.xml"}}, {"value": "0", "module": "A1-A3"}, {"value": "0", "module": "A4"}, {"value": "0", "module": "A5"}, {"value": "0", "module": "B2"}, {"value": "0", "module": "B6", "scenario": "S1"}, {"value": "0", "module": "B6", "scenario": "S2"}, {"value": "0", "module": "C1"}, {"value": "0", "module": "C2"}, {"value": "0", "module": "C3"}, {"value": "0", "module": "C4"}, {"value": "0", "module": "D"}]}, "resolvedFlowVersion": "38.00.000", "flowProperties": [], "typeOfFlow": "Other flow", "classification": {"classHierarchy": "Quantities / Environmental quantities / EPD EN 15804 / LCI indicators", "name": "GaBiCategories"}}, {"dataSetInternalID": 9, "referenceToFlowDataSet": {"shortDescription": [{"value": "Use of non renewable secondary fuels (NRSF)", "lang": "en"}, {"value": "Nicht erneuerbare Sekundärbrennstoffe (NRSF)", "lang": "de"}], "type": "flow data set", "refObjectId": "89def144-d39a-4287-b86f-efde453ddcb2", "uri": "../flows/89def144-d39a-4287-b86f-efde453ddcb2.xml"}, "exchange direction": "INPUT", "other": {"anies": [{"name": "referenceToUnitGroupDataSet", "value": {"shortDescription": [{"value": "MJ", "lang": "en"}], "type": "unit group data set", "refObjectId": "93a60a57-a3c8-11da-a746-0800200c9a66", "uri": "../unitgroups/93a60a57-a3c8-11da-a746-0800200c9a66.xml"}}, {"value": "0", "module": "A1-A3"}, {"value": "0", "module": "A4"}, {"value": "0", "module": "A5"}, {"value": "0", "module": "B2"}, {"value": "0", "module": "B6", "scenario": "S1"}, {"value": "0", "module": "B6", "scenario": "S2"}, {"value": "0", "module": "C1"}, {"value": "0", "module": "C2"}, {"value": "0", "module": "C3"}, {"value": "0", "module": "C4"}, {"value": "0", "module": "D"}]}, "resolvedFlowVersion": "38.00.000", "flowProperties": [], "typeOfFlow": "Other flow", "classification": {"classHierarchy": "Quantities / Environmental quantities / EPD EN 15804 / LCI indicators", "name": "GaBiCategories"}}, {"dataSetInternalID": 10, "referenceToFlowDataSet": {"shortDescription": [{"value": "Use of net fresh water (FW)", "lang": "en"}, {"value": "Einsatz von Süßwasserressourcen (FW)", "lang": "de"}], "type": "flow data set", "refObjectId": "3cf952c8-f3a4-461d-8c96-96456ca62246", "uri": "../flows/3cf952c8-f3a4-461d-8c96-96456ca62246.xml"}, "exchange direction": "INPUT", "other": {"anies": [{"name": "referenceToUnitGroupDataSet", "value": {"shortDescription": [{"value": "m^3", "lang": "en"}], "type": "unit group data set", "refObjectId": "cd950537-0a98-4044-9ba7-9f9a68d0a504", "uri": "../unitgroups/cd950537-0a98-4044-9ba7-9f9a68d0a504.xml"}}, {"value": "0.0756322", "module": "A1-A3"}, {"value": "6.74E-05", "module": "A4"}, {"value": "5.21E-05", "module": "A5"}, {"value": "0.00174", "module": "B2"}, {"value": "0.000137", "module": "B6", "scenario": "S1"}, {"value": "0.000136", "module": "B6", "scenario": "S2"}, {"value": "0", "module": "C1"}, {"value": "2.03E-07", "module": "C2"}, {"value": "0.000613", "module": "C3"}, {"value": "9.87E-07", "module": "C4"}, {"value": "-0.0172", "module": "D"}]}, "resolvedFlowVersion": "38.00.000", "flowProperties": [], "typeOfFlow": "Other flow", "classification": {"classHierarchy": "Quantities / Environmental quantities / EPD EN 15804 / LCI indicators", "name": "GaBiCategories"}}, {"dataSetInternalID": 11, "referenceToFlowDataSet": {"shortDescription": [{"value": "Hazardous waste disposed (HWD)", "lang": "en"}, {"value": "Gefährlicher Abfall zur Deponie (HWD)", "lang": "de"}], "type": "flow data set", "refObjectId": "430f9e0f-59b2-46a0-8e0d-55e0e84948fc", "uri": "../flows/430f9e0f-59b2-46a0-8e0d-55e0e84948fc.xml"}, "exchange direction": "OUTPUT", "other": {"anies": [{"name": "referenceToUnitGroupDataSet", "value": {"shortDescription": [{"value": "kg", "lang": "en"}], "type": "unit group data set", "refObjectId": "ad38d542-3fe9-439d-9b95-2f5f7752acaf", "uri": "../unitgroups/ad38d542-3fe9-439d-9b95-2f5f7752acaf.xml"}}, {"value": "2.095486E-06", "module": "A1-A3"}, {"value": "1.38E-09", "module": "A4"}, {"value": "8.31E-12", "module": "A5"}, {"value": "4.84E-08", "module": "B2"}, {"value": "1.11E-10", "module": "B6", "scenario": "S1"}, {"value": "1.34E-10", "module": "B6", "scenario": "S2"}, {"value": "0", "module": "C1"}, {"value": "3.49E-12", "module": "C2"}, {"value": "4.37E-10", "module": "C3"}, {"value": "5.97E-11", "module": "C4"}, {"value": "-5.94E-07", "module": "D"}]}, "resolvedFlowVersion": "38.00.000", "flowProperties": [], "typeOfFlow": "Other flow", "classification": {"classHierarchy": "Quantities / Environmental quantities / EPD EN 15804 / LCI indicators", "name": "GaBiCategories"}}, {"dataSetInternalID": 12, "referenceToFlowDataSet": {"shortDescription": [{"value": "Non hazardous waste disposed (NHWD)", "lang": "en"}, {"value": "Entsorgter nicht gefährlicher Abfall (NHWD)", "lang": "de"}], "type": "flow data set", "refObjectId": "b29ef66b-e286-4afa-949f-62f1a7b4d7fa", "uri": "../flows/b29ef66b-e286-4afa-949f-62f1a7b4d7fa.xml"}, "exchange direction": "OUTPUT", "other": {"anies": [{"name": "referenceToUnitGroupDataSet", "value": {"shortDescription": [{"value": "kg", "lang": "en"}], "type": "unit group data set", "refObjectId": "ad38d542-3fe9-439d-9b95-2f5f7752acaf", "uri": "../unitgroups/ad38d542-3fe9-439d-9b95-2f5f7752acaf.xml"}}, {"value": "0.371789", "module": "A1-A3"}, {"value": "0.00146", "module": "A4"}, {"value": "0.00056", "module": "A5"}, {"value": "0.0727", "module": "B2"}, {"value": "0.00019", "module": "B6", "scenario": "S1"}, {"value": "0.000118", "module": "B6", "scenario": "S2"}, {"value": "0", "module": "C1"}, {"value": "3.68E-06", "module": "C2"}, {"value": "0.0257", "module": "C3"}, {"value": "0.0197", "module": "C4"}, {"value": "0.00419", "module": "D"}]}, "resolvedFlowVersion": "38.00.000", "flowProperties": [], "typeOfFlow": "Other flow", "classification": {"classHierarchy": "Quantities / Environmental quantities / EPD EN 15804 / LCI indicators", "name": "GaBiCategories"}}, {"dataSetInternalID": 13, "referenceToFlowDataSet": {"shortDescription": [{"value": "Radioactive waste disposed (RWD)", "lang": "en"}, {"value": "Entsorgter radioaktiver Abfall (RWD)", "lang": "de"}], "type": "flow data set", "refObjectId": "3449546e-52ad-4b39-b809-9fb77cea8ff6", "uri": "../flows/3449546e-52ad-4b39-b809-9fb77cea8ff6.xml"}, "exchange direction": "OUTPUT", "other": {"anies": [{"name": "referenceToUnitGroupDataSet", "value": {"shortDescription": [{"value": "kg", "lang": "en"}], "type": "unit group data set", "refObjectId": "ad38d542-3fe9-439d-9b95-2f5f7752acaf", "uri": "../unitgroups/ad38d542-3fe9-439d-9b95-2f5f7752acaf.xml"}}, {"value": "0.00945561", "module": "A1-A3"}, {"value": "1.18E-05", "module": "A4"}, {"value": "2.96E-07", "module": "A5"}, {"value": "8.97E-05", "module": "B2"}, {"value": "4.06E-05", "module": "B6", "scenario": "S1"}, {"value": "2.77E-05", "module": "B6", "scenario": "S2"}, {"value": "0", "module": "C1"}, {"value": "3.86E-08", "module": "C2"}, {"value": "4.3E-06", "module": "C3"}, {"value": "4.46E-08", "module": "C4"}, {"value": "-0.00132", "module": "D"}]}, "resolvedFlowVersion": "38.00.000", "flowProperties": [], "typeOfFlow": "Other flow", "classification": {"classHierarchy": "Quantities / Environmental quantities / EPD EN 15804 / LCI indicators", "name": "GaBiCategories"}}, {"dataSetInternalID": 14, "referenceToFlowDataSet": {"shortDescription": [{"value": "Components for re-use (CRU)", "lang": "en"}, {"value": "Komponenten für die Wiederverwendung (CRU)", "lang": "de"}], "type": "flow data set", "refObjectId": "a2b32f97-3fc7-4af2-b209-525bc6426f33", "uri": "../flows/a2b32f97-3fc7-4af2-b209-525bc6426f33.xml"}, "exchange direction": "OUTPUT", "other": {"anies": [{"name": "referenceToUnitGroupDataSet", "value": {"shortDescription": [{"value": "kg", "lang": "en"}], "type": "unit group data set", "refObjectId": "ad38d542-3fe9-439d-9b95-2f5f7752acaf", "uri": "../unitgroups/ad38d542-3fe9-439d-9b95-2f5f7752acaf.xml"}}, {"value": "0", "module": "A1-A3"}, {"value": "0", "module": "A4"}, {"value": "0", "module": "A5"}, {"value": "0", "module": "B2"}, {"value": "0", "module": "B6", "scenario": "S1"}, {"value": "0", "module": "B6", "scenario": "S2"}, {"value": "0", "module": "C1"}, {"value": "0", "module": "C2"}, {"value": "0", "module": "C3"}, {"value": "0", "module": "C4"}, {"value": "0", "module": "D"}]}, "resolvedFlowVersion": "38.00.000", "flowProperties": [], "typeOfFlow": "Other flow", "classification": {"classHierarchy": "Quantities / Environmental quantities / EPD EN 15804 / LCI indicators", "name": "GaBiCategories"}}, {"dataSetInternalID": 15, "referenceToFlowDataSet": {"shortDescription": [{"value": "Materials for recycling (MFR)", "lang": "en"}, {"value": "Stoffe zum Recycling (MFR)", "lang": "de"}], "type": "flow data set", "refObjectId": "d7fe48a5-4103-49c8-9aae-b0b5dfdbd6ae", "uri": "../flows/d7fe48a5-4103-49c8-9aae-b0b5dfdbd6ae.xml"}, "exchange direction": "OUTPUT", "other": {"anies": [{"name": "referenceToUnitGroupDataSet", "value": {"shortDescription": [{"value": "kg", "lang": "en"}], "type": "unit group data set", "refObjectId": "ad38d542-3fe9-439d-9b95-2f5f7752acaf", "uri": "../unitgroups/ad38d542-3fe9-439d-9b95-2f5f7752acaf.xml"}}, {"value": "0", "module": "A1-A3"}, {"value": "0", "module": "A4"}, {"value": "0", "module": "A5"}, {"value": "0", "module": "B2"}, {"value": "0", "module": "B6", "scenario": "S1"}, {"value": "0", "module": "B6", "scenario": "S2"}, {"value": "0", "module": "C1"}, {"value": "0", "module": "C2"}, {"value": "0.487", "module": "C3"}, {"value": "0", "module": "C4"}, {"value": "0", "module": "D"}]}, "resolvedFlowVersion": "38.00.000", "flowProperties": [], "typeOfFlow": "Other flow", "classification": {"classHierarchy": "Quantities / Environmental quantities / EPD EN 15804 / LCI indicators", "name": "GaBiCategories"}}, {"dataSetInternalID": 16, "referenceToFlowDataSet": {"shortDescription": [{"value": "Materials for energy recovery (MER)", "lang": "en"}, {"value": "Stoffe für die Energierückgewinnung (MER)", "lang": "de"}], "type": "flow data set", "refObjectId": "59a9181c-3aaf-46ee-8b13-2b3723b6e447", "uri": "../flows/59a9181c-3aaf-46ee-8b13-2b3723b6e447.xml"}, "exchange direction": "OUTPUT", "other": {"anies": [{"name": "referenceToUnitGroupDataSet", "value": {"shortDescription": [{"value": "kg", "lang": "en"}], "type": "unit group data set", "refObjectId": "ad38d542-3fe9-439d-9b95-2f5f7752acaf", "uri": "../unitgroups/ad38d542-3fe9-439d-9b95-2f5f7752acaf.xml"}}, {"value": "0", "module": "A1-A3"}, {"value": "0", "module": "A4"}, {"value": "0", "module": "A5"}, {"value": "0", "module": "B2"}, {"value": "0", "module": "B6", "scenario": "S1"}, {"value": "0", "module": "B6", "scenario": "S2"}, {"value": "0", "module": "C1"}, {"value": "0", "module": "C2"}, {"value": "0", "module": "C3"}, {"value": "0", "module": "C4"}, {"value": "0", "module": "D"}]}, "resolvedFlowVersion": "38.00.000", "flowProperties": [], "typeOfFlow": "Other flow", "classification": {"classHierarchy": "Quantities / Environmental quantities / EPD EN 15804 / LCI indicators", "name": "GaBiCategories"}}, {"dataSetInternalID": 17, "referenceToFlowDataSet": {"shortDescription": [{"value": "Exported electrical energy (EEE)", "lang": "en"}, {"value": "Exportierte elektrische Energie (EEE)", "lang": "de"}], "type": "flow data set", "refObjectId": "4da0c987-2b76-40d6-9e9e-82a017aaaf29", "uri": "../flows/4da0c987-2b76-40d6-9e9e-82a017aaaf29.xml"}, "exchange direction": "OUTPUT", "other": {"anies": [{"name": "referenceToUnitGroupDataSet", "value": {"shortDescription": [{"value": "MJ", "lang": "en"}], "type": "unit group data set", "refObjectId": "93a60a57-a3c8-11da-a746-0800200c9a66", "uri": "../unitgroups/93a60a57-a3c8-11da-a746-0800200c9a66.xml"}}, {"value": "0.00247", "module": "A1-A3"}, {"value": "0", "module": "A4"}, {"value": "0.027", "module": "A5"}, {"value": "0", "module": "B2"}, {"value": "0", "module": "B6", "scenario": "S1"}, {"value": "0", "module": "B6", "scenario": "S2"}, {"value": "0", "module": "C1"}, {"value": "0", "module": "C2"}, {"value": "0", "module": "C3"}, {"value": "0", "module": "C4"}, {"value": "0", "module": "D"}]}, "resolvedFlowVersion": "38.00.000", "flowProperties": [], "typeOfFlow": "Other flow", "classification": {"classHierarchy": "Quantities / Environmental quantities / EPD EN 15804 / LCI indicators", "name": "GaBiCategories"}}, {"dataSetInternalID": 18, "referenceToFlowDataSet": {"shortDescription": [{"value": "Exported thermal energy (EET)", "lang": "en"}, {"value": "Exportierte thermische Energie (EET)", "lang": "de"}], "type": "flow data set", "refObjectId": "98daf38a-7a79-46d3-9a37-2b7bd0955810", "uri": "../flows/98daf38a-7a79-46d3-9a37-2b7bd0955810.xml"}, "exchange direction": "OUTPUT", "other": {"anies": [{"name": "referenceToUnitGroupDataSet", "value": {"shortDescription": [{"value": "MJ", "lang": "en"}], "type": "unit group data set", "refObjectId": "93a60a57-a3c8-11da-a746-0800200c9a66", "uri": "../unitgroups/93a60a57-a3c8-11da-a746-0800200c9a66.xml"}}, {"value": "0.00447", "module": "A1-A3"}, {"value": "0", "module": "A4"}, {"value": "0.049", "module": "A5"}, {"value": "0", "module": "B2"}, {"value": "0", "module": "B6", "scenario": "S1"}, {"value": "0", "module": "B6", "scenario": "S2"}, {"value": "0", "module": "C1"}, {"value": "0", "module": "C2"}, {"value": "0", "module": "C3"}, {"value": "0", "module": "C4"}, {"value": "0", "module": "D"}]}, "resolvedFlowVersion": "38.00.000", "flowProperties": [], "typeOfFlow": "Other flow", "classification": {"classHierarchy": "Quantities / Environmental quantities / EPD EN 15804 / LCI indicators", "name": "GaBiCategories"}}]}, "LCIAResults": {"LCIAResult": [{"referenceToLCIAMethodDataSet": {"shortDescription": [{"value": "Global Warming Potential total (GWP-total)", "lang": "en"}, {"value": "Globales Erwärmungspotenzial total (GWP-total)", "lang": "de"}], "type": "LCIA method data set", "refObjectId": "6a37f984-a4b3-458a-a20a-64418c145fa2", "uri": "../lciamethods/6a37f984-a4b3-458a-a20a-64418c145fa2.xml"}, "other": {"anies": [{"name": "referenceToUnitGroupDataSet", "value": {"shortDescription": [{"value": "kg CO_(2) eq", "lang": "en"}], "type": "unit group data set", "refObjectId": "1ebf3012-d0db-4de2-aefd-ef30cedb0be1", "uri": "../unitgroups/1ebf3012-d0db-4de2-aefd-ef30cedb0be1.xml"}}, {"value": "15.1424", "module": "A1-A3"}, {"value": "1.06", "module": "A4"}, {"value": "0.0179", "module": "A5"}, {"value": "0.3", "module": "B2"}, {"value": "0.0153", "module": "B6", "scenario": "S1"}, {"value": "0.0226", "module": "B6", "scenario": "S2"}, {"value": "0", "module": "C1"}, {"value": "0.00265", "module": "C2"}, {"value": "0.251", "module": "C3"}, {"value": "0.0003", "module": "C4"}, {"value": "-3.61", "module": "D"}]}}, {"referenceToLCIAMethodDataSet": {"shortDescription": [{"value": "Global Warming Potential fossil fuels (GWP-fossil)", "lang": "en"}, {"value": "Globales Erwärmungspotenzial fossil (GWP-fossil)", "lang": "de"}], "type": "LCIA method data set", "refObjectId": "5f635281-343e-44fb-83df-1971b155e6b6", "uri": "../lciamethods/5f635281-343e-44fb-83df-1971b155e6b6.xml"}, "other": {"anies": [{"name": "referenceToUnitGroupDataSet", "value": {"shortDescription": [{"value": "kg CO_(2) eq", "lang": "en"}], "type": "unit group data set", "refObjectId": "1ebf3012-d0db-4de2-aefd-ef30cedb0be1", "uri": "../unitgroups/1ebf3012-d0db-4de2-aefd-ef30cedb0be1.xml"}}, {"value": "15.0536", "module": "A1-A3"}, {"value": "1.06", "module": "A4"}, {"value": "0.000447", "module": "A5"}, {"value": "0.3", "module": "B2"}, {"value": "0.0152", "module": "B6", "scenario": "S1"}, {"value": "0.0226", "module": "B6", "scenario": "S2"}, {"value": "0", "module": "C1"}, {"value": "0.00253", "module": "C2"}, {"value": "0.247", "module": "C3"}, {"value": "0.000298", "module": "C4"}, {"value": "-3.6", "module": "D"}]}}, {"referenceToLCIAMethodDataSet": {"shortDescription": [{"value": "Global Warming Potential biogenic (GWP-biogenic)", "lang": "en"}, {"value": "Globales Erwärmungspotenzial biogen (GWP-biogenic)", "lang": "de"}], "type": "LCIA method data set", "refObjectId": "2356e1ab-0185-4db5-86e5-16de51c7485c", "uri": "../lciamethods/2356e1ab-0185-4db5-86e5-16de51c7485c.xml"}, "other": {"anies": [{"name": "referenceToUnitGroupDataSet", "value": {"shortDescription": [{"value": "kg CO_(2) eq", "lang": "en"}], "type": "unit group data set", "refObjectId": "1ebf3012-d0db-4de2-aefd-ef30cedb0be1", "uri": "../unitgroups/1ebf3012-d0db-4de2-aefd-ef30cedb0be1.xml"}}, {"value": "0.01724", "module": "A1-A3"}, {"value": "0.00178", "module": "A4"}, {"value": "0.0174", "module": "A5"}, {"value": "0.000526", "module": "B2"}, {"value": "5.07E-05", "module": "B6", "scenario": "S1"}, {"value": "9.48E-06", "module": "B6", "scenario": "S2"}, {"value": "0", "module": "C1"}, {"value": "0.000117", "module": "C2"}, {"value": "0.00395", "module": "C3"}, {"value": "1.02E-06", "module": "C4"}, {"value": "-0.00766", "module": "D"}]}}, {"referenceToLCIAMethodDataSet": {"shortDescription": [{"value": "Global Warming Potential luluc (GWP-luluc)", "lang": "en"}, {"value": "Globales Erwärmungspotenzial luluc (GWP-luluc)", "lang": "de"}], "type": "LCIA method data set", "refObjectId": "4331bbdb-978a-490d-8707-eeb047f01a55", "uri": "../lciamethods/4331bbdb-978a-490d-8707-eeb047f01a55.xml"}, "other": {"anies": [{"name": "referenceToUnitGroupDataSet", "value": {"shortDescription": [{"value": "kg CO_(2) eq", "lang": "en"}], "type": "unit group data set", "refObjectId": "1ebf3012-d0db-4de2-aefd-ef30cedb0be1", "uri": "../unitgroups/1ebf3012-d0db-4de2-aefd-ef30cedb0be1.xml"}}, {"value": "0.00864001", "module": "A1-A3"}, {"value": "2.22E-05", "module": "A4"}, {"value": "2.94E-07", "module": "A5"}, {"value": "0.000288", "module": "B2"}, {"value": "2.21E-05", "module": "B6", "scenario": "S1"}, {"value": "1.13E-05", "module": "B6", "scenario": "S2"}, {"value": "0", "module": "C1"}, {"value": "6.03E-08", "module": "C2"}, {"value": "1.4E-05", "module": "C3"}, {"value": "8.59E-07", "module": "C4"}, {"value": "-0.0015", "module": "D"}]}}, {"referenceToLCIAMethodDataSet": {"shortDescription": [{"value": "Depletion potential of the stratospheric ozone layer (ODP)", "lang": "en"}, {"value": "Abbau Potential der stratosphärischen Ozonschicht (ODP)", "lang": "de"}], "type": "LCIA method data set", "refObjectId": "b5c629d6-def3-11e6-bf01-fe55135034f3", "uri": "../lciamethods/b5c629d6-def3-11e6-bf01-fe55135034f3.xml"}, "other": {"anies": [{"name": "referenceToUnitGroupDataSet", "value": {"shortDescription": [{"value": "kg CFC11 eq", "lang": "en"}], "type": "unit group data set", "refObjectId": "d9e957c9-7309-4474-bf3a-7777df6c4e5b", "uri": "../unitgroups/d9e957c9-7309-4474-bf3a-7777df6c4e5b.xml"}}, {"value": "2.401390174E-10", "module": "A1-A3"}, {"value": "7.72E-17", "module": "A4"}, {"value": "3.22E-18", "module": "A5"}, {"value": "5.65E-12", "module": "B2"}, {"value": "3.35E-16", "module": "B6", "scenario": "S1"}, {"value": "1.09E-16", "module": "B6", "scenario": "S2"}, {"value": "0", "module": "C1"}, {"value": "2.68E-19", "module": "C2"}, {"value": "1.25E-16", "module": "C3"}, {"value": "1.11E-18", "module": "C4"}, {"value": "-1.18E-14", "module": "D"}]}}, {"referenceToLCIAMethodDataSet": {"shortDescription": [{"value": "Acidification potential of land and water (AP)", "lang": "en"}, {"value": "Versauerungspotenzial von Boden und Wasser (AP)", "lang": "de"}], "type": "LCIA method data set", "refObjectId": "b5c611c6-def3-11e6-bf01-fe55135034f3", "uri": "../lciamethods/b5c611c6-def3-11e6-bf01-fe55135034f3.xml"}, "other": {"anies": [{"name": "referenceToUnitGroupDataSet", "value": {"shortDescription": [{"value": "mol H^(+) eq", "lang": "en"}], "type": "unit group data set", "refObjectId": "42e089ac-92bf-4bf2-8ca1-5fc40d18f2ed", "uri": "../unitgroups/42e089ac-92bf-4bf2-8ca1-5fc40d18f2ed.xml"}}, {"value": "0.108627", "module": "A1-A3"}, {"value": "0.00432", "module": "A4"}, {"value": "5E-06", "module": "A5"}, {"value": "0.000936", "module": "B2"}, {"value": "3.36E-05", "module": "B6", "scenario": "S1"}, {"value": "6.32E-05", "module": "B6", "scenario": "S2"}, {"value": "0", "module": "C1"}, {"value": "2.54E-06", "module": "C2"}, {"value": "4.45E-05", "module": "C3"}, {"value": "2.14E-06", "module": "C4"}, {"value": "-0.041", "module": "D"}]}}, {"referenceToLCIAMethodDataSet": {"shortDescription": [{"value": "Eutrophication potential aquatic freshwater (EP-freshwater)", "lang": "en"}, {"value": "Eutrophierungspotenzial Süßwasser (EP-freshwater)", "lang": "de"}], "type": "LCIA method data set", "refObjectId": "b53ec18f-7377-4ad3-86eb-cc3f4f276b2b", "uri": "../lciamethods/b53ec18f-7377-4ad3-86eb-cc3f4f276b2b.xml"}, "other": {"anies": [{"name": "referenceToUnitGroupDataSet", "value": {"shortDescription": [{"value": "kg P eq", "lang": "en"}], "type": "unit group data set", "refObjectId": "0429039d-a61d-4590-ba67-aa4a20a810a1", "uri": "../unitgroups/0429039d-a61d-4590-ba67-aa4a20a810a1.xml"}}, {"value": "3.2631E-05", "module": "A1-A3"}, {"value": "1.74E-07", "module": "A4"}, {"value": "6.3E-10", "module": "A5"}, {"value": "4.81E-07", "module": "B2"}, {"value": "4.06E-08", "module": "B6", "scenario": "S1"}, {"value": "1.55E-08", "module": "B6", "scenario": "S2"}, {"value": "0", "module": "C1"}, {"value": "5.42E-10", "module": "C2"}, {"value": "1.99E-08", "module": "C3"}, {"value": "5.12E-10", "module": "C4"}, {"value": "-4.25E-06", "module": "D"}]}}, {"referenceToLCIAMethodDataSet": {"shortDescription": [{"value": "Eutrophication potential aquatic marine (EP-marine)", "lang": "en"}, {"value": "Eutrophierungspotenzial Salzwasser (EP-marine)", "lang": "de"}], "type": "LCIA method data set", "refObjectId": "b5c619fa-def3-11e6-bf01-fe55135034f3", "uri": "../lciamethods/b5c619fa-def3-11e6-bf01-fe55135034f3.xml"}, "other": {"anies": [{"name": "referenceToUnitGroupDataSet", "value": {"shortDescription": [{"value": "kg N eq", "lang": "en"}], "type": "unit group data set", "refObjectId": "d05bb823-ecdf-4686-8c40-bf1d9257859f", "uri": "../unitgroups/d05bb823-ecdf-4686-8c40-bf1d9257859f.xml"}}, {"value": "0.0158398", "module": "A1-A3"}, {"value": "0.00192", "module": "A4"}, {"value": "1.81E-06", "module": "A5"}, {"value": "0.000205", "module": "B2"}, {"value": "7.46E-06", "module": "B6", "scenario": "S1"}, {"value": "1.17E-05", "module": "B6", "scenario": "S2"}, {"value": "0", "module": "C1"}, {"value": "8.07E-07", "module": "C2"}, {"value": "1.01E-05", "module": "C3"}, {"value": "5.51E-07", "module": "C4"}, {"value": "-0.00508", "module": "D"}]}}, {"referenceToLCIAMethodDataSet": {"shortDescription": [{"value": "Eutrophication potential terrestrial (EP-terrestrial)", "lang": "en"}, {"value": "Eutrophierungspotenzial Land (EP-terrestrial)", "lang": "de"}], "type": "LCIA method data set", "refObjectId": "b5c614d2-def3-11e6-bf01-fe55135034f3", "uri": "../lciamethods/b5c614d2-def3-11e6-bf01-fe55135034f3.xml"}, "other": {"anies": [{"name": "referenceToUnitGroupDataSet", "value": {"shortDescription": [{"value": "mol N eq", "lang": "en"}], "type": "unit group data set", "refObjectId": "71b4d617-0ec9-4d3f-b65e-e438940c2401", "uri": "../unitgroups/71b4d617-0ec9-4d3f-b65e-e438940c2401.xml"}}, {"value": "0.170705", "module": "A1-A3"}, {"value": "0.0211", "module": "A4"}, {"value": "2.25E-05", "module": "A5"}, {"value": "0.00259", "module": "B2"}, {"value": "7.84E-05", "module": "B6", "scenario": "S1"}, {"value": "0.000127", "module": "B6", "scenario": "S2"}, {"value": "0", "module": "C1"}, {"value": "8.97E-06", "module": "C2"}, {"value": "0.000203", "module": "C3"}, {"value": "6.05E-06", "module": "C4"}, {"value": "-0.0553", "module": "D"}]}}, {"referenceToLCIAMethodDataSet": {"shortDescription": [{"value": "Formation potential of tropospheric ozone photochemical oxidants (POCP)", "lang": "en"}, {"value": "Bildungspotential für troposphärisches Ozon (POCP)", "lang": "de"}], "type": "LCIA method data set", "refObjectId": "b5c610fe-def3-11e6-bf01-fe55135034f3", "uri": "../lciamethods/b5c610fe-def3-11e6-bf01-fe55135034f3.xml"}, "other": {"anies": [{"name": "referenceToUnitGroupDataSet", "value": {"shortDescription": [{"value": "kg NMVOC eq", "lang": "en"}], "type": "unit group data set", "refObjectId": "d27c25f8-fbc1-44c6-b47b-4adbae4199c6", "uri": "../unitgroups/d27c25f8-fbc1-44c6-b47b-4adbae4199c6.xml"}}, {"value": "0.047281", "module": "A1-A3"}, {"value": "0.00548", "module": "A4"}, {"value": "4.79E-06", "module": "A5"}, {"value": "0.000563", "module": "B2"}, {"value": "2.04E-05", "module": "B6", "scenario": "S1"}, {"value": "3.37E-05", "module": "B6", "scenario": "S2"}, {"value": "0", "module": "C1"}, {"value": "2.28E-06", "module": "C2"}, {"value": "2.79E-05", "module": "C3"}, {"value": "1.67E-06", "module": "C4"}, {"value": "-0.016", "module": "D"}]}}, {"referenceToLCIAMethodDataSet": {"shortDescription": [{"value": "Abiotic depletion potential for non fossil resources (ADPE)", "lang": "en"}, {"value": "Potenzial für den abiotischen Abbau nicht fossiler Ressourcen (ADPE)", "lang": "de"}], "type": "LCIA method data set", "refObjectId": "b2ad6494-c78d-11e6-9d9d-cec0c932ce01", "uri": "../lciamethods/b2ad6494-c78d-11e6-9d9d-cec0c932ce01.xml"}, "other": {"anies": [{"name": "referenceToUnitGroupDataSet", "value": {"shortDescription": [{"value": "kg Sb eq", "lang": "en"}], "type": "unit group data set", "refObjectId": "54ccd2d9-a32a-4fc2-923d-f2c8c93e89d4", "uri": "../unitgroups/54ccd2d9-a32a-4fc2-923d-f2c8c93e89d4.xml"}}, {"value": "0.00408184492", "module": "A1-A3"}, {"value": "3.01E-08", "module": "A4"}, {"value": "5.09E-11", "module": "A5"}, {"value": "1.32E-06", "module": "B2"}, {"value": "4.4E-09", "module": "B6", "scenario": "S1"}, {"value": "3.97E-09", "module": "B6", "scenario": "S2"}, {"value": "0", "module": "C1"}, {"value": "7.6E-11", "module": "C2"}, {"value": "1.71E-09", "module": "C3"}, {"value": "2.68E-11", "module": "C4"}, {"value": "-0.00223", "module": "D"}]}}, {"referenceToLCIAMethodDataSet": {"shortDescription": [{"value": "Abiotic depletion potential for fossil resources (ADPF)", "lang": "en"}, {"value": "Potenzial für den abiotischen Abbau fossiler Brennstoffe (ADPF)", "lang": "de"}], "type": "LCIA method data set", "refObjectId": "b2ad6110-c78d-11e6-9d9d-cec0c932ce01", "uri": "../lciamethods/b2ad6110-c78d-11e6-9d9d-cec0c932ce01.xml"}, "other": {"anies": [{"name": "referenceToUnitGroupDataSet", "value": {"shortDescription": [{"value": "MJ", "lang": "en"}], "type": "unit group data set", "refObjectId": "93a60a57-a3c8-11da-a746-0800200c9a66", "uri": "../unitgroups/93a60a57-a3c8-11da-a746-0800200c9a66.xml"}}, {"value": "212.52", "module": "A1-A3"}, {"value": "14.4", "module": "A4"}, {"value": "0.00564", "module": "A5"}, {"value": "3.86", "module": "B2"}, {"value": "0.267", "module": "B6", "scenario": "S1"}, {"value": "0.341", "module": "B6", "scenario": "S2"}, {"value": "0", "module": "C1"}, {"value": "0.0359", "module": "C2"}, {"value": "0.115", "module": "C3"}, {"value": "0.00391", "module": "C4"}, {"value": "-41.1", "module": "D"}]}}, {"referenceToLCIAMethodDataSet": {"shortDescription": [{"value": "Water use (WDP)", "lang": "en"}, {"value": "Wassernutzung (WDP)", "lang": "de"}], "type": "LCIA method data set", "refObjectId": "b2ad66ce-c78d-11e6-9d9d-cec0c932ce01", "uri": "../lciamethods/b2ad66ce-c78d-11e6-9d9d-cec0c932ce01.xml"}, "other": {"anies": [{"name": "referenceToUnitGroupDataSet", "value": {"shortDescription": [{"value": "m^(3) world eq deprived", "lang": "en"}], "type": "unit group data set", "refObjectId": "6ae2df01-888e-46c8-b17d-49fa3869b476", "uri": "../unitgroups/6ae2df01-888e-46c8-b17d-49fa3869b476.xml"}}, {"value": "2.584624", "module": "A1-A3"}, {"value": "0.00161", "module": "A4"}, {"value": "0.00221", "module": "A5"}, {"value": "0.0403", "module": "B2"}, {"value": "0.00332", "module": "B6", "scenario": "S1"}, {"value": "0.00483", "module": "B6", "scenario": "S2"}, {"value": "0", "module": "C1"}, {"value": "4.97E-06", "module": "C2"}, {"value": "0.0257", "module": "C3"}, {"value": "3.13E-05", "module": "C4"}, {"value": "-0.584", "module": "D"}]}}, {"referenceToLCIAMethodDataSet": {"shortDescription": [{"value": "Incidence of disease due to PM emissions (PM)", "lang": "en"}, {"value": "Auftreten von Krankheiten aufgrund von Feinstaubemissionen (PM)", "lang": "de"}], "type": "LCIA method data set", "refObjectId": "b5c602c6-def3-11e6-bf01-fe55135034f3", "uri": "../lciamethods/b5c602c6-def3-11e6-bf01-fe55135034f3.xml"}, "other": {"anies": [{"name": "referenceToUnitGroupDataSet", "value": {"shortDescription": [{"value": "Disease incidence", "lang": "en"}], "type": "unit group data set", "refObjectId": "3883559b-648f-4afc-8ba2-0bd24f3affa3", "uri": "../unitgroups/3883559b-648f-4afc-8ba2-0bd24f3affa3.xml"}}, {"value": "1.0411E-06", "module": "A1-A3"}, {"value": "1.4E-08", "module": "A4"}, {"value": "2.77E-11", "module": "A5"}, {"value": "9.82E-09", "module": "B2"}, {"value": "2.82E-10", "module": "B6", "scenario": "S1"}, {"value": "7.54E-10", "module": "B6", "scenario": "S2"}, {"value": "0", "module": "C1"}, {"value": "1.33E-11", "module": "C2"}, {"value": "5.64E-10", "module": "C3"}, {"value": "2.65E-11", "module": "C4"}, {"value": "-3.7E-07", "module": "D"}]}}, {"referenceToLCIAMethodDataSet": {"shortDescription": [{"value": "Human exposure efficiency relative to U235 (IR)", "lang": "en"}, {"value": "Wirkung durch Exposition des Menschen mit U235 (IR)", "lang": "de"}], "type": "LCIA method data set", "refObjectId": "b5c632be-def3-11e6-bf01-fe55135034f3", "uri": "../lciamethods/b5c632be-def3-11e6-bf01-fe55135034f3.xml"}, "other": {"anies": [{"name": "referenceToUnitGroupDataSet", "value": {"shortDescription": [{"value": "kBq U235 eq", "lang": "en"}], "type": "unit group data set", "refObjectId": "456b05bf-1415-44a9-9993-02452f554c09", "uri": "../unitgroups/456b05bf-1415-44a9-9993-02452f554c09.xml"}}, {"value": "0.927469", "module": "A1-A3"}, {"value": "0.00161", "module": "A4"}, {"value": "4.59E-05", "module": "A5"}, {"value": "0.00882", "module": "B2"}, {"value": "0.00666", "module": "B6", "scenario": "S1"}, {"value": "0.00262", "module": "B6", "scenario": "S2"}, {"value": "0", "module": "C1"}, {"value": "5.52E-06", "module": "C2"}, {"value": "0.00039", "module": "C3"}, {"value": "4.59E-06", "module": "C4"}, {"value": "-0.138", "module": "D"}]}}, {"referenceToLCIAMethodDataSet": {"shortDescription": [{"value": "Comparative toxic unit for ecosystems (ETP-fw)", "lang": "en"}, {"value": "Toxizitätsvergleichseinheit für Ökosysteme (ETP-fw)", "lang": "de"}], "type": "LCIA method data set", "refObjectId": "ee1082d1-b0f7-43ca-a1f0-21e2a4a74511", "uri": "../lciamethods/ee1082d1-b0f7-43ca-a1f0-21e2a4a74511.xml"}, "other": {"anies": [{"name": "referenceToUnitGroupDataSet", "value": {"shortDescription": [{"value": "CTUe", "lang": "en"}], "type": "unit group data set", "refObjectId": "aa959ded-f1eb-4efb-9c5c-2d60be36b3e6", "uri": "../unitgroups/aa959ded-f1eb-4efb-9c5c-2d60be36b3e6.xml"}}, {"value": "122.043", "module": "A1-A3"}, {"value": "10.2", "module": "A4"}, {"value": "0.00268", "module": "A5"}, {"value": "13.2", "module": "B2"}, {"value": "0.114", "module": "B6", "scenario": "S1"}, {"value": "0.0986", "module": "B6", "scenario": "S2"}, {"value": "0", "module": "C1"}, {"value": "0.0255", "module": "C2"}, {"value": "0.0433", "module": "C3"}, {"value": "0.00224", "module": "C4"}, {"value": "-11.8", "module": "D"}]}}, {"referenceToLCIAMethodDataSet": {"shortDescription": [{"value": "Comparative toxic unit for humans (carcinogenic) (HTP-c)", "lang": "en"}, {"value": "Toxizitätsvergleichseinheit für Menschen (krebserregend) (HTP-c)", "lang": "de"}], "type": "LCIA method data set", "refObjectId": "2299222a-bbd8-474f-9d4f-4dd1f18aea7c", "uri": "../lciamethods/2299222a-bbd8-474f-9d4f-4dd1f18aea7c.xml"}, "other": {"anies": [{"name": "referenceToUnitGroupDataSet", "value": {"shortDescription": [{"value": "CTUh", "lang": "en"}], "type": "unit group data set", "refObjectId": "d4c9523e-2d7e-49fd-8469-998f547d3a70", "uri": "../unitgroups/d4c9523e-2d7e-49fd-8469-998f547d3a70.xml"}}, {"value": "5.3118E-09", "module": "A1-A3"}, {"value": "1.92E-10", "module": "A4"}, {"value": "1.42E-13", "module": "A5"}, {"value": "6.69E-11", "module": "B2"}, {"value": "3.16E-12", "module": "B6", "scenario": "S1"}, {"value": "2.73E-12", "module": "B6", "scenario": "S2"}, {"value": "0", "module": "C1"}, {"value": "4.79E-13", "module": "C2"}, {"value": "3.74E-12", "module": "C3"}, {"value": "3.31E-13", "module": "C4"}, {"value": "4.81E-09", "module": "D"}]}}, {"referenceToLCIAMethodDataSet": {"shortDescription": [{"value": "Comparative toxic unit for humans (noncarcinogenic) (HTP-nc)", "lang": "en"}, {"value": "Toxizitätsvergleichseinheit für Menschen (nicht krebserregend) (HTP-nc)", "lang": "de"}], "type": "LCIA method data set", "refObjectId": "3af763a5-b7a1-48c9-9cee-1f223481fcef", "uri": "../lciamethods/3af763a5-b7a1-48c9-9cee-1f223481fcef.xml"}, "other": {"anies": [{"name": "referenceToUnitGroupDataSet", "value": {"shortDescription": [{"value": "CTUh", "lang": "en"}], "type": "unit group data set", "refObjectId": "d4c9523e-2d7e-49fd-8469-998f547d3a70", "uri": "../unitgroups/d4c9523e-2d7e-49fd-8469-998f547d3a70.xml"}}, {"value": "3.7684E-07", "module": "A1-A3"}, {"value": "8.85E-09", "module": "A4"}, {"value": "6.13E-12", "module": "A5"}, {"value": "7.74E-09", "module": "B2"}, {"value": "1.16E-10", "module": "B6", "scenario": "S1"}, {"value": "1.07E-10", "module": "B6", "scenario": "S2"}, {"value": "0", "module": "C1"}, {"value": "2.05E-11", "module": "C2"}, {"value": "3.77E-10", "module": "C3"}, {"value": "3.65E-11", "module": "C4"}, {"value": "5.76E-07", "module": "D"}]}}, {"referenceToLCIAMethodDataSet": {"shortDescription": [{"value": "Soil quality index (SQP)", "lang": "en"}, {"value": "Bodenqualitätsindex (SQP)", "lang": "de"}], "type": "LCIA method data set", "refObjectId": "b2ad6890-c78d-11e6-9d9d-cec0c932ce01", "uri": "../lciamethods/b2ad6890-c78d-11e6-9d9d-cec0c932ce01.xml"}, "other": {"anies": [{"name": "referenceToUnitGroupDataSet", "value": {"shortDescription": [{"value": "SQP", "lang": "en"}], "type": "unit group data set", "refObjectId": "f130951c-e67f-4f7f-8dd4-665de3974e18", "uri": "../unitgroups/f130951c-e67f-4f7f-8dd4-665de3974e18.xml"}}, {"value": "50.476", "module": "A1-A3"}, {"value": "0.0294", "module": "A4"}, {"value": "0.0015", "module": "A5"}, {"value": "0.376", "module": "B2"}, {"value": "0.0852", "module": "B6", "scenario": "S1"}, {"value": "0.0393", "module": "B6", "scenario": "S2"}, {"value": "0", "module": "C1"}, {"value": "9.24E-05", "module": "C2"}, {"value": "0.0345", "module": "C3"}, {"value": "0.000816", "module": "C4"}, {"value": "-2.57", "module": "D"}]}}]}, "otherAttributes": {"{http://www.indata.network/EPD/2019}epd-version": "1.2"}, "version": "1.1", "locations": "../ILCDLocations.xml"}