{"processInformation": {"dataSetInformation": {"UUID": "cc4df46a-ba1b-4baa-80c0-58f812511d0a", "name": {"baseName": [{"value": "PU thermal insulation boards with mineral fleece facing", "lang": "en"}, {"value": "PU-Wärmedämmplatten mit Mineralvlieskaschierung", "lang": "de"}], "functionalUnitFlowProperties": [{"lang": "en"}]}, "classificationInformation": {"classification": [{"class": [{"value": "Dämmstoffe", "level": 0, "classId": "2"}, {"value": "Polyurethan-Hartschaum (PU)", "level": 1, "classId": "2.4"}, {"value": "PIR-Hartschaum", "level": 2, "classId": "2.4.04"}], "name": "OEKOBAU.DAT"}, {"class": [{"value": "02 Building products", "level": 0}, {"value": "Thermal insulation products", "level": 1}, {"value": "Insulating materials made of foam plastics", "level": 2}], "name": "IBUCategories"}]}, "generalComment": [{"value": "Factory made rigid polyurethane foam (PU) products are used for the thermal insulation of buildings. PU includes both PIR and PUR products. The products are manufactured in the form of boards without or with flexible facings. This Product Declaration covers PU insulation boards with mineral fleece facings on both sides.", "lang": "en"}, {"value": "Werkseitig hergestellte Polyurethan-Hartschaumprodukte (PU) werden für die Wärmedämmung von Gebäuden verwendet. PU umfasst sowohl PIR- als auch PUR-Produkte. Die Produkte werden in Form von Platten ohne oder mit flexiblen Deckschichten hergestellt. Diese Produktdeklaration bezieht sich auf PU-Dämmplatten mit beidseitigen Mineralvlies-Deckschichten.", "lang": "de"}]}, "quantitativeReference": {"referenceToReferenceFlow": [0]}, "time": {"referenceYear": 2024, "dataSetValidUntil": 2029, "other": {"anies": [{"name": "publicationDateOfEPD", "value": 1732838400000}]}}, "geography": {"locationOfOperationSupplyOrProduction": {"location": "DE"}}, "technology": {"technologyDescriptionAndIncludedProcesses": [{"value": "Polyurethane rigid foam insulation boards with flexible mineral fleece facings are produced in a continuous process on a double belt line. In this process, the polyurethane reaction mixture pours from a mixing head onto the bottom mineral fleece facing, where it foams up and glues – still within the line's pressure area – with the top mineral fleece facing. After passing the double belt line, the foam boards are cut to the desired dimensions. Quality assurance The declared products are subject to quality controls. Quality assurance is based on surveillance and certification by independent Notified Bodies. \nTechnical data: \nFor determining technical data, testing methods as stated in  EN 13165 are used. The gross density of PU insulation boards with mineral fleece facings for building construction is approx. 31 - 32 kg/m.\n\nDepending on their thickness, the boards obtain nominal thermal conductivity from 0.025 W/(m.K) to 0.028 W/(m.K). These levels are equivalent to thermal conductivity design values from 0.026 W/(m.K) up to 0.029 W/(m.K). In addition, the nominal value of the thermal resistance from RD = 4.29 (m.K)/W to 4.80 (m.K)/W and the thickness from 25 mm to 28 mm of the insulation board at RD = 1 (m.K)/W can be specified.\n\nNominal compressive stress at 10% deformation or compressive strength is 100 kPa (dh) or 150 kPa (ds) acc. to DIN 4108-10. Higher compressive strength is possible. Nominal tensile strength perpendicular to the insulation board plane is 40 kPa. Higher tensile strength is possible. The water vapour diffusion resistance factor  of polyurethane rigid foam is between 40 and 200 acc. to DIN 4108-4. Maximum moisture absorption of polyurethane rigid foam at diffusion and condensation is at approx. 6 % by volume. Water absorption at total immersion of a 60 mm thick PU insulation board with mineral fleece facings was measured at 1.3 % by volume after 28 days. Moisture absorption after freezing and thawing was between 2 % and 7 % by volume (measured at insulating material without facings). Polyurethane rigid foam is a distinctive thermosetting material and therefore cannot be melted. \nDeclared unit: \nThe declared unit is 1 m of installed PU thermal insulation board with mineral fleece facing (on both sides) and has the following specifications:", "lang": "en"}, {"value": "Werkseitig hergestellte Polyurethan-Hartschaumprodukte (PU) werden für die Wärmedämmung von Gebäuden verwendet. PU umfasst sowohl PIR- als auch PUR-Produkte. Die Produkte werden in Form von Platten ohne oder mit flexiblen Deckschichten hergestellt. Diese Produktdeklaration bezieht sich auf PU-Dämmplatten mit beidseitigen Mineralvlies-Deckschichten. \nTechnische Daten: \nFür die Bestimmung der technischen Daten werden die in der EN 13165 genannten Prüfverfahren verwendet. Die Rohdichte von PU-Dämmplatten mit Mineralvlies-Deckschichten für den Hochbau beträgt ca. 31 - 32 kg/m³. Je nach Dicke erreichen die Platten eine Nennwärmeleitfähigkeit von 0,025 W/(m.K) bis 0,028 W/(m.K). Diese Werte entsprechen den Bemessungswerten der Wärmeleitfähigkeit von 0,026 W/(m.K) bis 0,029 W/(m.K). Darüber hinaus kann der Nennwert des Wärmedurchlasswiderstandes von RD = 4,29 (m².K)/W bis 4,80 (m².K)/W und die Dicke der Dämmplatte von 25 mm bis 28 mm bei RD = 1 (m².K)/W angegeben werden. Die Nenndruckspannung bei 10% Verformung oder Druckfestigkeit beträgt 100 kPa (dh) oder 150 kPa (ds) nach DIN 4108-10. Eine höhere Druckfestigkeit ist möglich. Die nominale Zugfestigkeit senkrecht zur Dämmplattenebene beträgt 40 kPa. Eine höhere Zugfestigkeit ist möglich. Der Wasserdampfdiffusionswiderstandsfaktor µ von Polyurethan-Hartschaum liegt nach DIN 4108-4 zwischen 40 und 200. Die maximale Feuchtigkeitsaufnahme von Polyurethan-Hartschaum bei Diffusion und Kondensation liegt bei ca. 6 Volumenprozent. Die Wasseraufnahme bei vollständigem Eintauchen einer 60 mm dicken PU-Dämmplatte mit Mineralvlieskaschierung wurde nach 28 Tagen mit 1,3 Volumenprozent gemessen. Die Feuchtigkeitsaufnahme nach dem Einfrieren und Auftauen lag zwischen 2 und 7 Volumenprozent (gemessen am Dämmstoff ohne Deckschichten). Polyurethan-Hartschaum ist ein ausgeprägtes duroplastisches Material und kann daher nicht geschmolzen werden. \nDeklarierte Einheit: \nDie angegebene Einheit besteht aus 1 m² verlegter PU-Wärmedämmplatte mit Mineralvliesbeschichtung (beidseitig) und hat folgende Spezifikationen:", "lang": "de"}], "technologicalApplicability": [{"value": "The scope of application of PU rigid foam insulation materials includes thermal insulation in building construction (e.g. pitched roofs, flat roofs, floors, ceilings and exterior walls (inside and outside)).", "lang": "en"}, {"value": "Der Anwendungsbereich von PU-Hartschaum-Dämmstoffen umfasst die Wärmedämmung im Hochbau (z.B. Schrägdächer, Flachdächer, Böden, Decken und Außenwände (innen und außen)).", "lang": "de"}]}}, "modellingAndValidation": {"LCIMethodAndAllocation": {"typeOfDataSet": "EPD", "referenceToLCAMethodDetails": [{"shortDescription": [{"value": "Insulating materials made of foam plastics.pdf", "lang": "en"}], "type": "source data set", "refObjectId": "4d255a71-1f86-448e-81c2-7aa67abc7586"}], "other": {"anies": [{"name": "subType", "value": "average dataset"}]}}, "dataSourcesTreatmentAndRepresentativeness": {"referenceToDataSource": [{"shortDescription": [{"value": "GaBi Database (all versions)", "lang": "en"}], "type": "source data set", "refObjectId": "28d74cc0-db8b-4d7e-bc44-5f6d56ce0c4a"}, {"shortDescription": [{"value": "Sphera MLC (fka GaBi) CUP 2023.02", "lang": "en"}], "type": "source data set", "refObjectId": "cb600d3b-e85a-42b3-b059-5591e2757fbb"}], "useAdviceForDataSet": [{"value": "Scope: \nThis EPD applies to all declared products of the IVPUs member companies Karl Bachl GmbH & Co KG, Paul Bauder GmbH & Co KG, IKO Insulation BV, Kingspan Insulation GmbH & Co KG, Linzmeier Bauelemente GmbH, puren gmbh, Recticel NV/SA, Steinbacher Dmmstoff GmbH, Unilin Insulation bv. The IVPU represents more than 90% of the companies within the German polyurethane insulation products market. This EPD is based on weighted averages which have been determined on the basis of the single values originating from the factories of the aforementioned manufacturing companies (see section 3.1). \nSystem boundary: \nThe type of EPD according to EN15804 is cradle to gate with options, modules C1–C4, and module D. \nThe life cycle assessment considers the following steps of the life cycle:\n\nProduction and supply of raw materials (A1)\nTransporting raw materials (A2)\nProduction including packaging (A3)\nTransport to construction site (A4)\nInstallation in buildings (thermal treatment of packaging waste) (A5)\nTransport to End-of-Life (C2)\nWaste treatment: energy for shredders (C3)\nThermal treatment (PU foam) (C3)\nRecycling or use potentials beyond the systems boundary (D).", "lang": "en"}, {"value": "Gültigkeitsbereich: \nDiese EPD gilt für alle deklarierten Produkte der IVPU-Mitgliedsunternehmen Karl Bachl GmbH & Co KG, Paul Bauder GmbH & Co KG, IKO Insulation BV, Kingspan Insulation GmbH & Co KG, Linzmeier Bauelemente GmbH, puren gmbh, Recticel NV/SA, Steinbacher Dämmstoff GmbH, Unilin Insulation bv. Das IVPU vertritt mehr als 90% der Unternehmen auf dem deutschen Markt für Polyurethan-Dämmstoffe. Diese EPD basiert auf gewichteten Durchschnittswerten, die auf der Grundlage der Einzelwerte aus den Fabriken der oben genannten Herstellerunternehmen ermittelt wurden (siehe Abschnitt 3.1). \nSystemgrenze: \nDie Art der EPD nach EN15804 ist Cradle-to-Gate mit Optionen, Modulen C1-C4 und Modul D. Die Ökobilanz berücksichtigt die folgenden Schritte des Lebenszyklus: Produktion und Lieferung von Rohstoffen (A1) Transport von Rohstoffen (A2) Produktion einschließlich Verpackung (A3) Transport zur Baustelle (A4) Einbau in Gebäude (thermische Behandlung von Verpackungsabfällen) (A5) Transport zum End-of-Life (C2) Abfallbehandlung: Energie für Schredder (C3) Thermische Behandlung (PU-Schaum) (C3) Recycling oder Nutzungspotenziale außerhalb der Systemgrenze (D).", "lang": "de"}], "other": {"anies": [{"name": "referenceToOriginalEPD", "value": {"shortDescription": {"value": "PU thermal insulation boards with mineral fleece facing.pdf", "defaultValue": "PU thermal insulation boards with mineral fleece facing.pdf", "lstrings": [{"lang": "en", "value": "PU thermal insulation boards with mineral fleece facing.pdf"}]}, "type": "source data set", "uuid": {"uuid": "1177e9ea-141e-4253-81ea-bdce28713919"}, "refObjectId": "1177e9ea-141e-4253-81ea-bdce28713919", "resourceURLs": ["https://oekobaudat.de/OEKOBAU.DAT/resource/sources/1177e9ea-141e-4253-81ea-bdce28713919/PU_thermal_insulation_boards_with_mineral_fleece_facing_20300.pdf?version=00.01.000"]}}]}}, "validation": {"review": [{"referenceToNameOfReviewerAndInstitution": [{"shortDescription": [{"value": "Institut Bauen und Umwelt e. V.", "lang": "en"}], "type": "contact data set", "refObjectId": "d111dbec-b024-4be5-86c5-752d6eb2cf95", "uri": "../contacts/d111dbec-b024-4be5-86c5-752d6eb2cf95.xml"}], "type": "Accredited third party review"}]}, "complianceDeclarations": {"compliance": [{"referenceToComplianceSystem": {"shortDescription": [{"value": "DIN EN 15804+A2", "lang": "en"}], "type": "source data set", "refObjectId": "c0016b33-8cf7-415c-ac6e-deba0d21440d", "uri": "../sources/c0016b33-8cf7-415c-ac6e-deba0d21440d.xml"}}, {"referenceToComplianceSystem": {"shortDescription": [{"value": "ISO 14025", "lang": "en"}], "type": "source data set", "refObjectId": "4f2eb655-6e44-4874-a95a-e28f5442cd4d", "uri": "../sources/4f2eb655-6e44-4874-a95a-e28f5442cd4d.xml"}}]}}, "administrativeInformation": {"commissionerAndGoal": {"referenceToCommissioner": [{"shortDescription": [{"value": "Industrieverband Polyurethan-Hartschaum e.V.", "lang": "en"}], "type": "contact data set", "refObjectId": "61e847ad-7245-4eda-ad2c-75f901ca26f0", "uri": "../contacts/61e847ad-7245-4eda-ad2c-75f901ca26f0.xml"}]}, "dataGenerator": {"referenceToPersonOrEntityGeneratingTheDataSet": [{"shortDescription": [{"value": "Sphera Solutions GmbH", "lang": "en"}], "type": "contact data set", "refObjectId": "6e882050-12ae-4797-a5df-69674aa5b701", "uri": "../contacts/6e882050-12ae-4797-a5df-69674aa5b701.xml"}]}, "dataEntryBy": {"timeStamp": 1732838400000, "referenceToDataSetFormat": [{"shortDescription": [{"value": "ILCD Format", "lang": "en"}], "type": "source data set", "refObjectId": "a97a0155-0234-4b87-b4ce-a45da52f2a40", "uri": "../sources/a97a0155-0234-4b87-b4ce-a45da52f2a40.xml"}, {"shortDescription": [{"value": "EPD-Datenformaterweiterungen v1.2", "lang": "de"}, {"value": "EPD Data Format Extensions v1.2", "lang": "en"}], "type": "source data set", "refObjectId": "a29449fd-aa2f-4de8-b5d7-4b06b43c6fde", "uri": "../sources/a29449fd-aa2f-4de8-b5d7-4b06b43c6fde.xml"}]}, "publicationAndOwnership": {"dataSetVersion": "00.01.001", "referenceToRegistrationAuthority": {"shortDescription": [{"value": "Institut Bauen und Umwelt e. V.", "lang": "en"}], "type": "contact data set", "refObjectId": "d111dbec-b024-4be5-86c5-752d6eb2cf95", "uri": "../contacts/d111dbec-b024-4be5-86c5-752d6eb2cf95.xml"}, "registrationNumber": "EPD-IVP-20240423-IBE1-EN", "referenceToOwnershipOfDataSet": {"shortDescription": [{"value": "Industrieverband Polyurethan-Hartschaum e.V.", "lang": "en"}], "type": "contact data set", "refObjectId": "61e847ad-7245-4eda-ad2c-75f901ca26f0", "uri": "../contacts/61e847ad-7245-4eda-ad2c-75f901ca26f0.xml"}, "copyright": true, "licenseType": "Free of charge for all users and uses", "accessRestrictions": [{"value": "None", "lang": "en"}], "other": {"anies": [{"name": "referenceToPublisher", "value": {"shortDescription": [{"value": "Institut Bauen und Umwelt e. V.", "lang": "en"}], "type": "contact data set", "refObjectId": "d111dbec-b024-4be5-86c5-752d6eb2cf95", "uri": "../contacts/d111dbec-b024-4be5-86c5-752d6eb2cf95.xml"}}]}}}, "exchanges": {"exchange": [{"dataSetInternalID": 0, "referenceToFlowDataSet": {"shortDescription": [{"value": "PU thermal insulation boards with mineral fleece facing ()", "lang": "en"}], "type": "flow data set", "refObjectId": "36e44fd6-4c08-c49d-8617-186279701997", "uri": "../flows/36e44fd6-4c08-c49d-8617-186279701997.xml"}, "meanAmount": 1.0, "referencesToDataSource": {}, "referenceFlow": true, "resolvedFlowVersion": "00.01.000", "resultingflowAmount": 1.0, "flowProperties": [{"name": [{"lang": "de", "value": "Fläche"}, {"lang": "en", "value": "Area"}], "uuid": "93a60a56-a3c8-19da-a746-0800200c9a66", "referenceFlowProperty": true, "meanValue": 1.0, "referenceUnit": "qm", "unitGroupUUID": "c20a03d7-bd90-4569-bc94-66cfd364dfc8"}], "materialProperties": [{"name": "layer thickness", "value": "0.12", "unit": "m", "unitDescription": "meters"}, {"name": "gross density", "value": "31.12", "unit": "kg/m^3", "unitDescription": "kilograms per cubic metre"}, {"name": "grammage", "value": "4.42", "unit": "kg/m^2", "unitDescription": "kilograms per square meter"}], "typeOfFlow": "Product flow", "classification": {"classHierarchy": "Dämmstoffe / Polyurethan-Hartschaum (PU) / PIR-Hartschaum", "name": "OEKOBAU.DAT"}}, {"dataSetInternalID": 1, "referenceToFlowDataSet": {"shortDescription": [{"value": "Renewable primary energy as energy carrier (PERE)", "lang": "en"}, {"value": "Erneuerbare Primärenergie als Energieträger (PERE)", "lang": "de"}], "type": "flow data set", "refObjectId": "20f32be5-0398-4288-9b6d-accddd195317", "uri": "../flows/20f32be5-0398-4288-9b6d-accddd195317.xml"}, "exchange direction": "INPUT", "other": {"anies": [{"name": "referenceToUnitGroupDataSet", "value": {"shortDescription": [{"value": "MJ", "lang": "en"}], "type": "unit group data set", "refObjectId": "93a60a57-a3c8-11da-a746-0800200c9a66", "uri": "../unitgroups/93a60a57-a3c8-11da-a746-0800200c9a66.xml"}}, {"value": "15.9007534731231", "module": "A1-A3"}, {"value": "0.471117237489889", "module": "A4"}, {"value": "1.35848860566644", "module": "A5"}, {"value": "0", "module": "C1"}, {"value": "0.0926429535959148", "module": "C2"}, {"value": "1.41494401027718", "module": "C3"}, {"value": "0.0198357624625441", "module": "C4"}, {"value": "-16.9922848866001", "module": "D"}]}, "resolvedFlowVersion": "38.00.000", "flowProperties": [], "typeOfFlow": "Other flow", "classification": {"classHierarchy": "Quantities", "name": "GaBiCategories"}}, {"dataSetInternalID": 2, "referenceToFlowDataSet": {"shortDescription": [{"value": "Renewable primary energy resources as material utilization (PERM)", "lang": "en"}, {"value": "Erneuerbare Primärenergie zur stofflichen Nutzung (PERM)", "lang": "de"}], "type": "flow data set", "refObjectId": "fb3ec0de-548d-4508-aea5-00b73bf6f702", "uri": "../flows/fb3ec0de-548d-4508-aea5-00b73bf6f702.xml"}, "exchange direction": "INPUT", "other": {"anies": [{"name": "referenceToUnitGroupDataSet", "value": {"shortDescription": [{"value": "MJ", "lang": "en"}], "type": "unit group data set", "refObjectId": "93a60a57-a3c8-11da-a746-0800200c9a66", "uri": "../unitgroups/93a60a57-a3c8-11da-a746-0800200c9a66.xml"}}, {"value": "1.35223068042", "module": "A1-A3"}, {"value": "0", "module": "A4"}, {"value": "-1.35223068042", "module": "A5"}, {"value": "0", "module": "C1"}, {"value": "0", "module": "C2"}, {"value": "0", "module": "C3"}, {"value": "0", "module": "C4"}, {"value": "0", "module": "D"}]}, "resolvedFlowVersion": "38.00.000", "flowProperties": [], "typeOfFlow": "Other flow", "classification": {"classHierarchy": "Quantities", "name": "GaBiCategories"}}, {"dataSetInternalID": 3, "referenceToFlowDataSet": {"shortDescription": [{"value": "Total use of renewable primary energy resources (PERT)", "lang": "en"}, {"value": "Total erneuerbare Primärenergie (PERT)", "lang": "de"}], "type": "flow data set", "refObjectId": "53f97275-fa8a-4cdd-9024-65936002acd0", "uri": "../flows/53f97275-fa8a-4cdd-9024-65936002acd0.xml"}, "exchange direction": "INPUT", "other": {"anies": [{"name": "referenceToUnitGroupDataSet", "value": {"shortDescription": [{"value": "MJ", "lang": "en"}], "type": "unit group data set", "refObjectId": "93a60a57-a3c8-11da-a746-0800200c9a66", "uri": "../unitgroups/93a60a57-a3c8-11da-a746-0800200c9a66.xml"}}, {"value": "17.2529841535431", "module": "A1-A3"}, {"value": "0.471117237489889", "module": "A4"}, {"value": "0.0062579252464408", "module": "A5"}, {"value": "0", "module": "C1"}, {"value": "0.0926429535959148", "module": "C2"}, {"value": "1.41494401027718", "module": "C3"}, {"value": "0.0198357624625441", "module": "C4"}, {"value": "-16.9922848866001", "module": "D"}]}, "resolvedFlowVersion": "38.00.000", "flowProperties": [], "typeOfFlow": "Other flow", "classification": {"classHierarchy": "Quantities / Environmental quantities / EPD EN 15804 / LCI indicators", "name": "GaBiCategories"}}, {"dataSetInternalID": 4, "referenceToFlowDataSet": {"shortDescription": [{"value": "Non renewable primary energy as energy carrier (PENRE)", "lang": "en"}, {"value": "Nicht-erneuerbare Primärenergie als Energieträger (PENRE)", "lang": "de"}], "type": "flow data set", "refObjectId": "ac857178-2b45-46ec-892a-a9a4332f0372", "uri": "../flows/ac857178-2b45-46ec-892a-a9a4332f0372.xml"}, "exchange direction": "INPUT", "other": {"anies": [{"name": "referenceToUnitGroupDataSet", "value": {"shortDescription": [{"value": "MJ", "lang": "en"}], "type": "unit group data set", "refObjectId": "93a60a57-a3c8-11da-a746-0800200c9a66", "uri": "../unitgroups/93a60a57-a3c8-11da-a746-0800200c9a66.xml"}}, {"value": "196.131543772037", "module": "A1-A3"}, {"value": "6.67383813440127", "module": "A4"}, {"value": "23.280134434515", "module": "A5"}, {"value": "0", "module": "C1"}, {"value": "1.31237837928877", "module": "C2"}, {"value": "99.1064248546252", "module": "C3"}, {"value": "0.121799956904978", "module": "C4"}, {"value": "-58.3345397978173", "module": "D"}]}, "resolvedFlowVersion": "38.00.000", "flowProperties": [], "typeOfFlow": "Other flow", "classification": {"classHierarchy": "Quantities", "name": "GaBiCategories"}}, {"dataSetInternalID": 5, "referenceToFlowDataSet": {"shortDescription": [{"value": "Non renewable primary energy as material utilization (PENRM)", "lang": "en"}, {"value": "Nicht-erneuerbare Primärenergie zur stofflichen Nutzung (PENRM)", "lang": "de"}], "type": "flow data set", "refObjectId": "1421caa0-679d-4bf4-b282-0eb850ccae27", "uri": "../flows/1421caa0-679d-4bf4-b282-0eb850ccae27.xml"}, "exchange direction": "INPUT", "other": {"anies": [{"name": "referenceToUnitGroupDataSet", "value": {"shortDescription": [{"value": "MJ", "lang": "en"}], "type": "unit group data set", "refObjectId": "93a60a57-a3c8-11da-a746-0800200c9a66", "uri": "../unitgroups/93a60a57-a3c8-11da-a746-0800200c9a66.xml"}}, {"value": "118.479717314", "module": "A1-A3"}, {"value": "0", "module": "A4"}, {"value": "-23.255078409", "module": "A5"}, {"value": "0", "module": "C1"}, {"value": "0", "module": "C2"}, {"value": "-95.224638905", "module": "C3"}, {"value": "0", "module": "C4"}, {"value": "0", "module": "D"}]}, "resolvedFlowVersion": "38.00.000", "flowProperties": [], "typeOfFlow": "Other flow", "classification": {"classHierarchy": "Quantities", "name": "GaBiCategories"}}, {"dataSetInternalID": 6, "referenceToFlowDataSet": {"shortDescription": [{"value": "Total use of non renewable primary energy resources (PENRT)", "lang": "en"}, {"value": "Total nicht erneuerbare Primärenergie (PENRT)", "lang": "de"}], "type": "flow data set", "refObjectId": "06159210-646b-4c8d-8583-da9b3b95a6c1", "uri": "../flows/06159210-646b-4c8d-8583-da9b3b95a6c1.xml"}, "exchange direction": "INPUT", "other": {"anies": [{"name": "referenceToUnitGroupDataSet", "value": {"shortDescription": [{"value": "MJ", "lang": "en"}], "type": "unit group data set", "refObjectId": "93a60a57-a3c8-11da-a746-0800200c9a66", "uri": "../unitgroups/93a60a57-a3c8-11da-a746-0800200c9a66.xml"}}, {"value": "314.611261086098", "module": "A1-A3"}, {"value": "6.67383813440127", "module": "A4"}, {"value": "0.0250560255150293", "module": "A5"}, {"value": "0", "module": "C1"}, {"value": "1.31237837928877", "module": "C2"}, {"value": "3.88178594962515", "module": "C3"}, {"value": "0.121799956904978", "module": "C4"}, {"value": "-58.3345397978174", "module": "D"}]}, "resolvedFlowVersion": "38.00.000", "flowProperties": [], "typeOfFlow": "Other flow", "classification": {"classHierarchy": "Quantities / Environmental quantities / EPD EN 15804 / LCI indicators", "name": "GaBiCategories"}}, {"dataSetInternalID": 7, "referenceToFlowDataSet": {"shortDescription": [{"value": "Use of secondary material (SM)", "lang": "en"}, {"value": "Einsatz von Sekundärstoffen (SM)", "lang": "de"}], "type": "flow data set", "refObjectId": "c6a1f35f-2d09-4f54-8dfb-97e502e1ce92", "uri": "../flows/c6a1f35f-2d09-4f54-8dfb-97e502e1ce92.xml"}, "exchange direction": "INPUT", "other": {"anies": [{"name": "referenceToUnitGroupDataSet", "value": {"shortDescription": [{"value": "kg", "lang": "en"}], "type": "unit group data set", "refObjectId": "ad38d542-3fe9-439d-9b95-2f5f7752acaf", "uri": "../unitgroups/ad38d542-3fe9-439d-9b95-2f5f7752acaf.xml"}}, {"value": "0", "module": "A1-A3"}, {"value": "0", "module": "A4"}, {"value": "0", "module": "A5"}, {"value": "0", "module": "C1"}, {"value": "0", "module": "C2"}, {"value": "0", "module": "C3"}, {"value": "0", "module": "C4"}, {"value": "0", "module": "D"}]}, "resolvedFlowVersion": "38.00.000", "flowProperties": [], "typeOfFlow": "Other flow", "classification": {"classHierarchy": "Quantities / Environmental quantities / EPD EN 15804 / LCI indicators", "name": "GaBiCategories"}}, {"dataSetInternalID": 8, "referenceToFlowDataSet": {"shortDescription": [{"value": "Use of renewable secondary fuels (RSF)", "lang": "en"}, {"value": "Erneuerbare Sekundärbrennstoffe (RSF)", "lang": "de"}], "type": "flow data set", "refObjectId": "64333088-a55f-4aa2-9a31-c10b07816787", "uri": "../flows/64333088-a55f-4aa2-9a31-c10b07816787.xml"}, "exchange direction": "INPUT", "other": {"anies": [{"name": "referenceToUnitGroupDataSet", "value": {"shortDescription": [{"value": "MJ", "lang": "en"}], "type": "unit group data set", "refObjectId": "93a60a57-a3c8-11da-a746-0800200c9a66", "uri": "../unitgroups/93a60a57-a3c8-11da-a746-0800200c9a66.xml"}}, {"value": "0", "module": "A1-A3"}, {"value": "0", "module": "A4"}, {"value": "0", "module": "A5"}, {"value": "0", "module": "C1"}, {"value": "0", "module": "C2"}, {"value": "0", "module": "C3"}, {"value": "0", "module": "C4"}, {"value": "0", "module": "D"}]}, "resolvedFlowVersion": "38.00.000", "flowProperties": [], "typeOfFlow": "Other flow", "classification": {"classHierarchy": "Quantities / Environmental quantities / EPD EN 15804 / LCI indicators", "name": "GaBiCategories"}}, {"dataSetInternalID": 9, "referenceToFlowDataSet": {"shortDescription": [{"value": "Use of non renewable secondary fuels (NRSF)", "lang": "en"}, {"value": "Nicht erneuerbare Sekundärbrennstoffe (NRSF)", "lang": "de"}], "type": "flow data set", "refObjectId": "89def144-d39a-4287-b86f-efde453ddcb2", "uri": "../flows/89def144-d39a-4287-b86f-efde453ddcb2.xml"}, "exchange direction": "INPUT", "other": {"anies": [{"name": "referenceToUnitGroupDataSet", "value": {"shortDescription": [{"value": "MJ", "lang": "en"}], "type": "unit group data set", "refObjectId": "93a60a57-a3c8-11da-a746-0800200c9a66", "uri": "../unitgroups/93a60a57-a3c8-11da-a746-0800200c9a66.xml"}}, {"value": "0", "module": "A1-A3"}, {"value": "0", "module": "A4"}, {"value": "0", "module": "A5"}, {"value": "0", "module": "C1"}, {"value": "0", "module": "C2"}, {"value": "0", "module": "C3"}, {"value": "0", "module": "C4"}, {"value": "0", "module": "D"}]}, "resolvedFlowVersion": "38.00.000", "flowProperties": [], "typeOfFlow": "Other flow", "classification": {"classHierarchy": "Quantities / Environmental quantities / EPD EN 15804 / LCI indicators", "name": "GaBiCategories"}}, {"dataSetInternalID": 10, "referenceToFlowDataSet": {"shortDescription": [{"value": "Use of net fresh water (FW)", "lang": "en"}, {"value": "Einsatz von Süßwasserressourcen (FW)", "lang": "de"}], "type": "flow data set", "refObjectId": "3cf952c8-f3a4-461d-8c96-96456ca62246", "uri": "../flows/3cf952c8-f3a4-461d-8c96-96456ca62246.xml"}, "exchange direction": "INPUT", "other": {"anies": [{"name": "referenceToUnitGroupDataSet", "value": {"shortDescription": [{"value": "m^3", "lang": "en"}], "type": "unit group data set", "refObjectId": "cd950537-0a98-4044-9ba7-9f9a68d0a504", "uri": "../unitgroups/cd950537-0a98-4044-9ba7-9f9a68d0a504.xml"}}, {"value": "0.0771010544926423", "module": "A1-A3"}, {"value": "0.000519155908138974", "module": "A4"}, {"value": "0.000428120220987589", "module": "A5"}, {"value": "0", "module": "C1"}, {"value": "0.000102089528634144", "module": "C2"}, {"value": "0.0203183696882763", "module": "C3"}, {"value": "3.07485499332323E-05", "module": "C4"}, {"value": "-0.0137671098078602", "module": "D"}]}, "resolvedFlowVersion": "38.00.000", "flowProperties": [], "typeOfFlow": "Other flow", "classification": {"classHierarchy": "Quantities / Environmental quantities / EPD EN 15804 / LCI indicators", "name": "GaBiCategories"}}, {"dataSetInternalID": 11, "referenceToFlowDataSet": {"shortDescription": [{"value": "Hazardous waste disposed (HWD)", "lang": "en"}, {"value": "Gefährlicher Abfall zur Deponie (HWD)", "lang": "de"}], "type": "flow data set", "refObjectId": "430f9e0f-59b2-46a0-8e0d-55e0e84948fc", "uri": "../flows/430f9e0f-59b2-46a0-8e0d-55e0e84948fc.xml"}, "exchange direction": "OUTPUT", "other": {"anies": [{"name": "referenceToUnitGroupDataSet", "value": {"shortDescription": [{"value": "kg", "lang": "en"}], "type": "unit group data set", "refObjectId": "ad38d542-3fe9-439d-9b95-2f5f7752acaf", "uri": "../unitgroups/ad38d542-3fe9-439d-9b95-2f5f7752acaf.xml"}}, {"value": "9.84202430512426E-08", "module": "A1-A3"}, {"value": "2.46939838574804E-11", "module": "A4"}, {"value": "6.81687457475037E-13", "module": "A5"}, {"value": "0", "module": "C1"}, {"value": "4.85595392942065E-12", "module": "C2"}, {"value": "6.3028561961218E-11", "module": "C3"}, {"value": "2.65034815465339E-12", "module": "C4"}, {"value": "-3.14713666677662E-09", "module": "D"}]}, "resolvedFlowVersion": "38.00.000", "flowProperties": [], "typeOfFlow": "Other flow", "classification": {"classHierarchy": "Quantities / Environmental quantities / EPD EN 15804 / LCI indicators", "name": "GaBiCategories"}}, {"dataSetInternalID": 12, "referenceToFlowDataSet": {"shortDescription": [{"value": "Non hazardous waste disposed (NHWD)", "lang": "en"}, {"value": "Entsorgter nicht gefährlicher Abfall (NHWD)", "lang": "de"}], "type": "flow data set", "refObjectId": "b29ef66b-e286-4afa-949f-62f1a7b4d7fa", "uri": "../flows/b29ef66b-e286-4afa-949f-62f1a7b4d7fa.xml"}, "exchange direction": "OUTPUT", "other": {"anies": [{"name": "referenceToUnitGroupDataSet", "value": {"shortDescription": [{"value": "kg", "lang": "en"}], "type": "unit group data set", "refObjectId": "ad38d542-3fe9-439d-9b95-2f5f7752acaf", "uri": "../unitgroups/ad38d542-3fe9-439d-9b95-2f5f7752acaf.xml"}}, {"value": "0.260618072670171", "module": "A1-A3"}, {"value": "0.000961868408661158", "module": "A4"}, {"value": "0.000842076328036618", "module": "A5"}, {"value": "0", "module": "C1"}, {"value": "0.000189146826432741", "module": "C2"}, {"value": "0.0435707908593882", "module": "C3"}, {"value": "0.609003052062604", "module": "C4"}, {"value": "-0.028825262249022", "module": "D"}]}, "resolvedFlowVersion": "38.00.000", "flowProperties": [], "typeOfFlow": "Other flow", "classification": {"classHierarchy": "Quantities / Environmental quantities / EPD EN 15804 / LCI indicators", "name": "GaBiCategories"}}, {"dataSetInternalID": 13, "referenceToFlowDataSet": {"shortDescription": [{"value": "Radioactive waste disposed (RWD)", "lang": "en"}, {"value": "Entsorgter radioaktiver Abfall (RWD)", "lang": "de"}], "type": "flow data set", "refObjectId": "3449546e-52ad-4b39-b809-9fb77cea8ff6", "uri": "../flows/3449546e-52ad-4b39-b809-9fb77cea8ff6.xml"}, "exchange direction": "OUTPUT", "other": {"anies": [{"name": "referenceToUnitGroupDataSet", "value": {"shortDescription": [{"value": "kg", "lang": "en"}], "type": "unit group data set", "refObjectId": "ad38d542-3fe9-439d-9b95-2f5f7752acaf", "uri": "../unitgroups/ad38d542-3fe9-439d-9b95-2f5f7752acaf.xml"}}, {"value": "0.00435842502923602", "module": "A1-A3"}, {"value": "8.62891892049001E-06", "module": "A4"}, {"value": "1.47084830823036E-06", "module": "A5"}, {"value": "0", "module": "C1"}, {"value": "1.69683567384016E-06", "module": "C2"}, {"value": "0.000355384062523103", "module": "C3"}, {"value": "1.38868199255962E-06", "module": "C4"}, {"value": "-0.00450861301744451", "module": "D"}]}, "resolvedFlowVersion": "38.00.000", "flowProperties": [], "typeOfFlow": "Other flow", "classification": {"classHierarchy": "Quantities / Environmental quantities / EPD EN 15804 / LCI indicators", "name": "GaBiCategories"}}, {"dataSetInternalID": 14, "referenceToFlowDataSet": {"shortDescription": [{"value": "Components for re-use (CRU)", "lang": "en"}, {"value": "Komponenten für die Wiederverwendung (CRU)", "lang": "de"}], "type": "flow data set", "refObjectId": "a2b32f97-3fc7-4af2-b209-525bc6426f33", "uri": "../flows/a2b32f97-3fc7-4af2-b209-525bc6426f33.xml"}, "exchange direction": "OUTPUT", "other": {"anies": [{"name": "referenceToUnitGroupDataSet", "value": {"shortDescription": [{"value": "kg", "lang": "en"}], "type": "unit group data set", "refObjectId": "ad38d542-3fe9-439d-9b95-2f5f7752acaf", "uri": "../unitgroups/ad38d542-3fe9-439d-9b95-2f5f7752acaf.xml"}}, {"value": "0", "module": "A1-A3"}, {"value": "0", "module": "A4"}, {"value": "0", "module": "A5"}, {"value": "0", "module": "C1"}, {"value": "0", "module": "C2"}, {"value": "0", "module": "C3"}, {"value": "0", "module": "C4"}, {"value": "0", "module": "D"}]}, "resolvedFlowVersion": "38.00.000", "flowProperties": [], "typeOfFlow": "Other flow", "classification": {"classHierarchy": "Quantities / Environmental quantities / EPD EN 15804 / LCI indicators", "name": "GaBiCategories"}}, {"dataSetInternalID": 15, "referenceToFlowDataSet": {"shortDescription": [{"value": "Materials for recycling (MFR)", "lang": "en"}, {"value": "Stoffe zum Recycling (MFR)", "lang": "de"}], "type": "flow data set", "refObjectId": "d7fe48a5-4103-49c8-9aae-b0b5dfdbd6ae", "uri": "../flows/d7fe48a5-4103-49c8-9aae-b0b5dfdbd6ae.xml"}, "exchange direction": "OUTPUT", "other": {"anies": [{"name": "referenceToUnitGroupDataSet", "value": {"shortDescription": [{"value": "kg", "lang": "en"}], "type": "unit group data set", "refObjectId": "ad38d542-3fe9-439d-9b95-2f5f7752acaf", "uri": "../unitgroups/ad38d542-3fe9-439d-9b95-2f5f7752acaf.xml"}}, {"value": "0", "module": "A1-A3"}, {"value": "0", "module": "A4"}, {"value": "0", "module": "A5"}, {"value": "0", "module": "C1"}, {"value": "0", "module": "C2"}, {"value": "0", "module": "C3"}, {"value": "0", "module": "C4"}, {"value": "0", "module": "D"}]}, "resolvedFlowVersion": "38.00.000", "flowProperties": [], "typeOfFlow": "Other flow", "classification": {"classHierarchy": "Quantities / Environmental quantities / EPD EN 15804 / LCI indicators", "name": "GaBiCategories"}}, {"dataSetInternalID": 16, "referenceToFlowDataSet": {"shortDescription": [{"value": "Materials for energy recovery (MER)", "lang": "en"}, {"value": "Stoffe für die Energierückgewinnung (MER)", "lang": "de"}], "type": "flow data set", "refObjectId": "59a9181c-3aaf-46ee-8b13-2b3723b6e447", "uri": "../flows/59a9181c-3aaf-46ee-8b13-2b3723b6e447.xml"}, "exchange direction": "OUTPUT", "other": {"anies": [{"name": "referenceToUnitGroupDataSet", "value": {"shortDescription": [{"value": "kg", "lang": "en"}], "type": "unit group data set", "refObjectId": "ad38d542-3fe9-439d-9b95-2f5f7752acaf", "uri": "../unitgroups/ad38d542-3fe9-439d-9b95-2f5f7752acaf.xml"}}, {"value": "0", "module": "A1-A3"}, {"value": "0", "module": "A4"}, {"value": "0", "module": "A5"}, {"value": "0", "module": "C1"}, {"value": "0", "module": "C2"}, {"value": "0", "module": "C3"}, {"value": "0", "module": "C4"}, {"value": "0", "module": "D"}]}, "resolvedFlowVersion": "38.00.000", "flowProperties": [], "typeOfFlow": "Other flow", "classification": {"classHierarchy": "Quantities / Environmental quantities / EPD EN 15804 / LCI indicators", "name": "GaBiCategories"}}, {"dataSetInternalID": 17, "referenceToFlowDataSet": {"shortDescription": [{"value": "Exported electrical energy (EEE)", "lang": "en"}, {"value": "Exportierte elektrische Energie (EEE)", "lang": "de"}], "type": "flow data set", "refObjectId": "4da0c987-2b76-40d6-9e9e-82a017aaaf29", "uri": "../flows/4da0c987-2b76-40d6-9e9e-82a017aaaf29.xml"}, "exchange direction": "OUTPUT", "other": {"anies": [{"name": "referenceToUnitGroupDataSet", "value": {"shortDescription": [{"value": "MJ", "lang": "en"}], "type": "unit group data set", "refObjectId": "93a60a57-a3c8-11da-a746-0800200c9a66", "uri": "../unitgroups/93a60a57-a3c8-11da-a746-0800200c9a66.xml"}}, {"value": "0", "module": "A1-A3"}, {"value": "0", "module": "A4"}, {"value": "0.412672213125171", "module": "A5"}, {"value": "0", "module": "C1"}, {"value": "0", "module": "C2"}, {"value": "14.5911272343205", "module": "C3"}, {"value": "0", "module": "C4"}, {"value": "0", "module": "D"}]}, "resolvedFlowVersion": "38.00.000", "flowProperties": [], "typeOfFlow": "Other flow", "classification": {"classHierarchy": "Quantities / Environmental quantities / EPD EN 15804 / LCI indicators", "name": "GaBiCategories"}}, {"dataSetInternalID": 18, "referenceToFlowDataSet": {"shortDescription": [{"value": "Exported thermal energy (EET)", "lang": "en"}, {"value": "Exportierte thermische Energie (EET)", "lang": "de"}], "type": "flow data set", "refObjectId": "98daf38a-7a79-46d3-9a37-2b7bd0955810", "uri": "../flows/98daf38a-7a79-46d3-9a37-2b7bd0955810.xml"}, "exchange direction": "OUTPUT", "other": {"anies": [{"name": "referenceToUnitGroupDataSet", "value": {"shortDescription": [{"value": "MJ", "lang": "en"}], "type": "unit group data set", "refObjectId": "93a60a57-a3c8-11da-a746-0800200c9a66", "uri": "../unitgroups/93a60a57-a3c8-11da-a746-0800200c9a66.xml"}}, {"value": "0", "module": "A1-A3"}, {"value": "0", "module": "A4"}, {"value": "0.734299557738438", "module": "A5"}, {"value": "0", "module": "C1"}, {"value": "0", "module": "C2"}, {"value": "26.2476673269461", "module": "C3"}, {"value": "0", "module": "C4"}, {"value": "0", "module": "D"}]}, "resolvedFlowVersion": "38.00.000", "flowProperties": [], "typeOfFlow": "Other flow", "classification": {"classHierarchy": "Quantities / Environmental quantities / EPD EN 15804 / LCI indicators", "name": "GaBiCategories"}}]}, "LCIAResults": {"LCIAResult": [{"referenceToLCIAMethodDataSet": {"shortDescription": [{"value": "Global Warming Potential total (GWP-total)", "lang": "en"}, {"value": "Globales Erwärmungspotenzial total (GWP-total)", "lang": "de"}], "type": "LCIA method data set", "refObjectId": "6a37f984-a4b3-458a-a20a-64418c145fa2", "uri": "../lciamethods/6a37f984-a4b3-458a-a20a-64418c145fa2.xml"}, "other": {"anies": [{"name": "referenceToUnitGroupDataSet", "value": {"shortDescription": [{"value": "kg CO_(2) eq", "lang": "en"}], "type": "unit group data set", "refObjectId": "1ebf3012-d0db-4de2-aefd-ef30cedb0be1", "uri": "../unitgroups/1ebf3012-d0db-4de2-aefd-ef30cedb0be1.xml"}}, {"value": "12.0442144581066", "module": "A1-A3"}, {"value": "0.485159884165714", "module": "A4"}, {"value": "0.203419764890606", "module": "A5"}, {"value": "0", "module": "C1"}, {"value": "0.0954043729642313", "module": "C2"}, {"value": "8.5246834442694", "module": "C3"}, {"value": "0.00903588673147948", "module": "C4"}, {"value": "-3.17023001446002", "module": "D"}]}}, {"referenceToLCIAMethodDataSet": {"shortDescription": [{"value": "Global Warming Potential fossil fuels (GWP-fossil)", "lang": "en"}, {"value": "Globales Erwärmungspotenzial fossil (GWP-fossil)", "lang": "de"}], "type": "LCIA method data set", "refObjectId": "5f635281-343e-44fb-83df-1971b155e6b6", "uri": "../lciamethods/5f635281-343e-44fb-83df-1971b155e6b6.xml"}, "other": {"anies": [{"name": "referenceToUnitGroupDataSet", "value": {"shortDescription": [{"value": "kg CO_(2) eq", "lang": "en"}], "type": "unit group data set", "refObjectId": "1ebf3012-d0db-4de2-aefd-ef30cedb0be1", "uri": "../unitgroups/1ebf3012-d0db-4de2-aefd-ef30cedb0be1.xml"}}, {"value": "12.0710613346262", "module": "A1-A3"}, {"value": "0.479505253888501", "module": "A4"}, {"value": "0.201234450373557", "module": "A5"}, {"value": "0", "module": "C1"}, {"value": "0.094292416939941", "module": "C2"}, {"value": "8.52349057835134", "module": "C3"}, {"value": "0.00900722090891361", "module": "C4"}, {"value": "-3.15554777435469", "module": "D"}]}}, {"referenceToLCIAMethodDataSet": {"shortDescription": [{"value": "Global Warming Potential biogenic (GWP-biogenic)", "lang": "en"}, {"value": "Globales Erwärmungspotenzial biogen (GWP-biogenic)", "lang": "de"}], "type": "LCIA method data set", "refObjectId": "2356e1ab-0185-4db5-86e5-16de51c7485c", "uri": "../lciamethods/2356e1ab-0185-4db5-86e5-16de51c7485c.xml"}, "other": {"anies": [{"name": "referenceToUnitGroupDataSet", "value": {"shortDescription": [{"value": "kg CO_(2) eq", "lang": "en"}], "type": "unit group data set", "refObjectId": "1ebf3012-d0db-4de2-aefd-ef30cedb0be1", "uri": "../unitgroups/1ebf3012-d0db-4de2-aefd-ef30cedb0be1.xml"}}, {"value": "-0.0373426897710223", "module": "A1-A3"}, {"value": "0.00112068711614913", "module": "A4"}, {"value": "0.00218510579356714", "module": "A5"}, {"value": "0", "module": "C1"}, {"value": "0.000220377766371098", "module": "C2"}, {"value": "0.00117077040876213", "module": "C3"}, {"value": "2.70543748273318E-07", "module": "C4"}, {"value": "-0.0144758706820739", "module": "D"}]}}, {"referenceToLCIAMethodDataSet": {"shortDescription": [{"value": "Global Warming Potential luluc (GWP-luluc)", "lang": "en"}, {"value": "Globales Erwärmungspotenzial luluc (GWP-luluc)", "lang": "de"}], "type": "LCIA method data set", "refObjectId": "4331bbdb-978a-490d-8707-eeb047f01a55", "uri": "../lciamethods/4331bbdb-978a-490d-8707-eeb047f01a55.xml"}, "other": {"anies": [{"name": "referenceToUnitGroupDataSet", "value": {"shortDescription": [{"value": "kg CO_(2) eq", "lang": "en"}], "type": "unit group data set", "refObjectId": "1ebf3012-d0db-4de2-aefd-ef30cedb0be1", "uri": "../unitgroups/1ebf3012-d0db-4de2-aefd-ef30cedb0be1.xml"}}, {"value": "0.0104958132514735", "module": "A1-A3"}, {"value": "0.00453394316106359", "module": "A4"}, {"value": "2.08723482567174E-07", "module": "A5"}, {"value": "0", "module": "C1"}, {"value": "0.000891578257919177", "module": "C2"}, {"value": "2.20955093003174E-05", "module": "C3"}, {"value": "2.83952788175974E-05", "module": "C4"}, {"value": "-0.000206369423263285", "module": "D"}]}}, {"referenceToLCIAMethodDataSet": {"shortDescription": [{"value": "Depletion potential of the stratospheric ozone layer (ODP)", "lang": "en"}, {"value": "Abbau Potential der stratosphärischen Ozonschicht (ODP)", "lang": "de"}], "type": "LCIA method data set", "refObjectId": "b5c629d6-def3-11e6-bf01-fe55135034f3", "uri": "../lciamethods/b5c629d6-def3-11e6-bf01-fe55135034f3.xml"}, "other": {"anies": [{"name": "referenceToUnitGroupDataSet", "value": {"shortDescription": [{"value": "kg CFC11 eq", "lang": "en"}], "type": "unit group data set", "refObjectId": "d9e957c9-7309-4474-bf3a-7777df6c4e5b", "uri": "../unitgroups/d9e957c9-7309-4474-bf3a-7777df6c4e5b.xml"}}, {"value": "1.44986887178122E-11", "module": "A1-A3"}, {"value": "4.28600594948124E-14", "module": "A4"}, {"value": "9.80055242806298E-15", "module": "A5"}, {"value": "0", "module": "C1"}, {"value": "8.42822589988819E-15", "module": "C2"}, {"value": "2.14403810147978E-12", "module": "C3"}, {"value": "2.32471026646794E-14", "module": "C4"}, {"value": "-2.48860546040749E-11", "module": "D"}]}}, {"referenceToLCIAMethodDataSet": {"shortDescription": [{"value": "Acidification potential of land and water (AP)", "lang": "en"}, {"value": "Versauerungspotenzial von Boden und Wasser (AP)", "lang": "de"}], "type": "LCIA method data set", "refObjectId": "b5c611c6-def3-11e6-bf01-fe55135034f3", "uri": "../lciamethods/b5c611c6-def3-11e6-bf01-fe55135034f3.xml"}, "other": {"anies": [{"name": "referenceToUnitGroupDataSet", "value": {"shortDescription": [{"value": "mol H^(+) eq", "lang": "en"}], "type": "unit group data set", "refObjectId": "42e089ac-92bf-4bf2-8ca1-5fc40d18f2ed", "uri": "../unitgroups/42e089ac-92bf-4bf2-8ca1-5fc40d18f2ed.xml"}}, {"value": "0.0234893352383497", "module": "A1-A3"}, {"value": "0.000638508735987998", "module": "A4"}, {"value": "2.29468313541813E-05", "module": "A5"}, {"value": "0", "module": "C1"}, {"value": "0.000125559691922739", "module": "C2"}, {"value": "0.00506881782174303", "module": "C3"}, {"value": "6.48234769422265E-05", "module": "C4"}, {"value": "-0.00395471311411294", "module": "D"}]}}, {"referenceToLCIAMethodDataSet": {"shortDescription": [{"value": "Eutrophication potential aquatic freshwater (EP-freshwater)", "lang": "en"}, {"value": "Eutrophierungspotenzial Süßwasser (EP-freshwater)", "lang": "de"}], "type": "LCIA method data set", "refObjectId": "b53ec18f-7377-4ad3-86eb-cc3f4f276b2b", "uri": "../lciamethods/b53ec18f-7377-4ad3-86eb-cc3f4f276b2b.xml"}, "other": {"anies": [{"name": "referenceToUnitGroupDataSet", "value": {"shortDescription": [{"value": "kg P eq", "lang": "en"}], "type": "unit group data set", "refObjectId": "0429039d-a61d-4590-ba67-aa4a20a810a1", "uri": "../unitgroups/0429039d-a61d-4590-ba67-aa4a20a810a1.xml"}}, {"value": "4.7484146146732E-05", "module": "A1-A3"}, {"value": "1.78500435274728E-06", "module": "A4"}, {"value": "2.35801161137886E-09", "module": "A5"}, {"value": "0", "module": "C1"}, {"value": "3.51012576617135E-07", "module": "C2"}, {"value": "4.80437710861584E-07", "module": "C3"}, {"value": "1.84044798110754E-08", "module": "C4"}, {"value": "-5.13386202605046E-06", "module": "D"}]}}, {"referenceToLCIAMethodDataSet": {"shortDescription": [{"value": "Eutrophication potential aquatic marine (EP-marine)", "lang": "en"}, {"value": "Eutrophierungspotenzial Salzwasser (EP-marine)", "lang": "de"}], "type": "LCIA method data set", "refObjectId": "b5c619fa-def3-11e6-bf01-fe55135034f3", "uri": "../lciamethods/b5c619fa-def3-11e6-bf01-fe55135034f3.xml"}, "other": {"anies": [{"name": "referenceToUnitGroupDataSet", "value": {"shortDescription": [{"value": "kg N eq", "lang": "en"}], "type": "unit group data set", "refObjectId": "d05bb823-ecdf-4686-8c40-bf1d9257859f", "uri": "../unitgroups/d05bb823-ecdf-4686-8c40-bf1d9257859f.xml"}}, {"value": "0.00638449635383615", "module": "A1-A3"}, {"value": "0.000224791609728099", "module": "A4"}, {"value": "5.97950455364007E-06", "module": "A5"}, {"value": "0", "module": "C1"}, {"value": "4.42041959231819E-05", "module": "C2"}, {"value": "0.00240827765412861", "module": "C3"}, {"value": "1.67493656574772E-05", "module": "C4"}, {"value": "-0.0011564606176276", "module": "D"}]}}, {"referenceToLCIAMethodDataSet": {"shortDescription": [{"value": "Eutrophication potential terrestrial (EP-terrestrial)", "lang": "en"}, {"value": "Eutrophierungspotenzial Land (EP-terrestrial)", "lang": "de"}], "type": "LCIA method data set", "refObjectId": "b5c614d2-def3-11e6-bf01-fe55135034f3", "uri": "../lciamethods/b5c614d2-def3-11e6-bf01-fe55135034f3.xml"}, "other": {"anies": [{"name": "referenceToUnitGroupDataSet", "value": {"shortDescription": [{"value": "mol N eq", "lang": "en"}], "type": "unit group data set", "refObjectId": "71b4d617-0ec9-4d3f-b65e-e438940c2401", "uri": "../unitgroups/71b4d617-0ec9-4d3f-b65e-e438940c2401.xml"}}, {"value": "0.065910986440585", "module": "A1-A3"}, {"value": "0.00269889897698891", "module": "A4"}, {"value": "0.000111418313357556", "module": "A5"}, {"value": "0", "module": "C1"}, {"value": "0.000530725587578637", "module": "C2"}, {"value": "0.0277398200071049", "module": "C3"}, {"value": "0.000184284843640454", "module": "C4"}, {"value": "-0.0123808595808396", "module": "D"}]}}, {"referenceToLCIAMethodDataSet": {"shortDescription": [{"value": "Formation potential of tropospheric ozone photochemical oxidants (POCP)", "lang": "en"}, {"value": "Bildungspotential für troposphärisches Ozon (POCP)", "lang": "de"}], "type": "LCIA method data set", "refObjectId": "b5c610fe-def3-11e6-bf01-fe55135034f3", "uri": "../lciamethods/b5c610fe-def3-11e6-bf01-fe55135034f3.xml"}, "other": {"anies": [{"name": "referenceToUnitGroupDataSet", "value": {"shortDescription": [{"value": "kg NMVOC eq", "lang": "en"}], "type": "unit group data set", "refObjectId": "d27c25f8-fbc1-44c6-b47b-4adbae4199c6", "uri": "../unitgroups/d27c25f8-fbc1-44c6-b47b-4adbae4199c6.xml"}}, {"value": "0.0347617410235326", "module": "A1-A3"}, {"value": "0.000551395918692587", "module": "A4"}, {"value": "1.69466016631948E-05", "module": "A5"}, {"value": "0", "module": "C1"}, {"value": "0.00010842937265591", "module": "C2"}, {"value": "0.00618825793410055", "module": "C3"}, {"value": "5.05426197636554E-05", "module": "C4"}, {"value": "-0.00321981278078887", "module": "D"}]}}, {"referenceToLCIAMethodDataSet": {"shortDescription": [{"value": "Abiotic depletion potential for non fossil resources (ADPE)", "lang": "en"}, {"value": "Potenzial für den abiotischen Abbau nicht fossiler Ressourcen (ADPE)", "lang": "de"}], "type": "LCIA method data set", "refObjectId": "b2ad6494-c78d-11e6-9d9d-cec0c932ce01", "uri": "../lciamethods/b2ad6494-c78d-11e6-9d9d-cec0c932ce01.xml"}, "other": {"anies": [{"name": "referenceToUnitGroupDataSet", "value": {"shortDescription": [{"value": "kg Sb eq", "lang": "en"}], "type": "unit group data set", "refObjectId": "54ccd2d9-a32a-4fc2-923d-f2c8c93e89d4", "uri": "../unitgroups/54ccd2d9-a32a-4fc2-923d-f2c8c93e89d4.xml"}}, {"value": "1.2960266632862E-06", "module": "A1-A3"}, {"value": "3.17947559320366E-08", "module": "A4"}, {"value": "9.12503810038663E-11", "module": "A5"}, {"value": "0", "module": "C1"}, {"value": "6.25228682800706E-09", "module": "C2"}, {"value": "1.87106848808092E-08", "module": "C3"}, {"value": "4.2251167471594E-10", "module": "C4"}, {"value": "-2.27315904472689E-07", "module": "D"}]}}, {"referenceToLCIAMethodDataSet": {"shortDescription": [{"value": "Abiotic depletion potential for fossil resources (ADPF)", "lang": "en"}, {"value": "Potenzial für den abiotischen Abbau fossiler Brennstoffe (ADPF)", "lang": "de"}], "type": "LCIA method data set", "refObjectId": "b2ad6110-c78d-11e6-9d9d-cec0c932ce01", "uri": "../lciamethods/b2ad6110-c78d-11e6-9d9d-cec0c932ce01.xml"}, "other": {"anies": [{"name": "referenceToUnitGroupDataSet", "value": {"shortDescription": [{"value": "MJ", "lang": "en"}], "type": "unit group data set", "refObjectId": "93a60a57-a3c8-11da-a746-0800200c9a66", "uri": "../unitgroups/93a60a57-a3c8-11da-a746-0800200c9a66.xml"}}, {"value": "314.396524177124", "module": "A1-A3"}, {"value": "6.65671372674402", "module": "A4"}, {"value": "0.0250355306763975", "module": "A5"}, {"value": "0", "module": "C1"}, {"value": "1.30901094634915", "module": "C2"}, {"value": "3.88017154178673", "module": "C3"}, {"value": "0.121662790273642", "module": "C4"}, {"value": "-58.3268497065084", "module": "D"}]}}, {"referenceToLCIAMethodDataSet": {"shortDescription": [{"value": "Water use (WDP)", "lang": "en"}, {"value": "Wassernutzung (WDP)", "lang": "de"}], "type": "LCIA method data set", "refObjectId": "b2ad66ce-c78d-11e6-9d9d-cec0c932ce01", "uri": "../lciamethods/b2ad66ce-c78d-11e6-9d9d-cec0c932ce01.xml"}, "other": {"anies": [{"name": "referenceToUnitGroupDataSet", "value": {"shortDescription": [{"value": "m^(3) world eq deprived", "lang": "en"}], "type": "unit group data set", "refObjectId": "6ae2df01-888e-46c8-b17d-49fa3869b476", "uri": "../unitgroups/6ae2df01-888e-46c8-b17d-49fa3869b476.xml"}}, {"value": "1.78488716411567", "module": "A1-A3"}, {"value": "0.00564227519870225", "module": "A4"}, {"value": "0.018273797220084", "module": "A5"}, {"value": "0", "module": "C1"}, {"value": "0.00110952645713793", "module": "C2"}, {"value": "0.847702708876161", "module": "C3"}, {"value": "0.0010034613768657", "module": "C4"}, {"value": "-0.301473494298307", "module": "D"}]}}, {"referenceToLCIAMethodDataSet": {"shortDescription": [{"value": "Incidence of disease due to PM emissions (PM)", "lang": "en"}, {"value": "Auftreten von Krankheiten aufgrund von Feinstaubemissionen (PM)", "lang": "de"}], "type": "LCIA method data set", "refObjectId": "b5c602c6-def3-11e6-bf01-fe55135034f3", "uri": "../lciamethods/b5c602c6-def3-11e6-bf01-fe55135034f3.xml"}, "other": {"anies": [{"name": "referenceToUnitGroupDataSet", "value": {"shortDescription": [{"value": "Disease incidence", "lang": "en"}], "type": "unit group data set", "refObjectId": "3883559b-648f-4afc-8ba2-0bd24f3affa3", "uri": "../unitgroups/3883559b-648f-4afc-8ba2-0bd24f3affa3.xml"}}, {"value": "2.01365195099977E-07", "module": "A1-A3"}, {"value": "5.30230846039677E-09", "module": "A4"}, {"value": "1.22274059590949E-10", "module": "A5"}, {"value": "0", "module": "C1"}, {"value": "1.04267362252545E-09", "module": "C2"}, {"value": "1.50911603932173E-08", "module": "C3"}, {"value": "7.9728362846092E-10", "module": "C4"}, {"value": "-3.34721777142589E-08", "module": "D"}]}}, {"referenceToLCIAMethodDataSet": {"shortDescription": [{"value": "Human exposure efficiency relative to U235 (IR)", "lang": "en"}, {"value": "Wirkung durch Exposition des Menschen mit U235 (IR)", "lang": "de"}], "type": "LCIA method data set", "refObjectId": "b5c632be-def3-11e6-bf01-fe55135034f3", "uri": "../lciamethods/b5c632be-def3-11e6-bf01-fe55135034f3.xml"}, "other": {"anies": [{"name": "referenceToUnitGroupDataSet", "value": {"shortDescription": [{"value": "kBq U235 eq", "lang": "en"}], "type": "unit group data set", "refObjectId": "456b05bf-1415-44a9-9993-02452f554c09", "uri": "../unitgroups/456b05bf-1415-44a9-9993-02452f554c09.xml"}}, {"value": "0.434730329387534", "module": "A1-A3"}, {"value": "0.0012454170553028", "module": "A4"}, {"value": "0.000237260107355931", "module": "A5"}, {"value": "0", "module": "C1"}, {"value": "0.000244905312904103", "module": "C2"}, {"value": "0.0583414977043471", "module": "C3"}, {"value": "0.00016044805148494", "module": "C4"}, {"value": "-0.749983064635796", "module": "D"}]}}, {"referenceToLCIAMethodDataSet": {"shortDescription": [{"value": "Comparative toxic unit for ecosystems (ETP-fw)", "lang": "en"}, {"value": "Toxizitätsvergleichseinheit für Ökosysteme (ETP-fw)", "lang": "de"}], "type": "LCIA method data set", "refObjectId": "ee1082d1-b0f7-43ca-a1f0-21e2a4a74511", "uri": "../lciamethods/ee1082d1-b0f7-43ca-a1f0-21e2a4a74511.xml"}, "other": {"anies": [{"name": "referenceToUnitGroupDataSet", "value": {"shortDescription": [{"value": "CTUe", "lang": "en"}], "type": "unit group data set", "refObjectId": "aa959ded-f1eb-4efb-9c5c-2d60be36b3e6", "uri": "../unitgroups/aa959ded-f1eb-4efb-9c5c-2d60be36b3e6.xml"}}, {"value": "108.237442555369", "module": "A1-A3"}, {"value": "4.68834958808623", "module": "A4"}, {"value": "0.00965898195009712", "module": "A5"}, {"value": "0", "module": "C1"}, {"value": "0.921941543987384", "module": "C2"}, {"value": "1.11143274110631", "module": "C3"}, {"value": "0.0658349732275981", "module": "C4"}, {"value": "-8.13661927316375", "module": "D"}]}}, {"referenceToLCIAMethodDataSet": {"shortDescription": [{"value": "Comparative toxic unit for humans (carcinogenic) (HTP-c)", "lang": "en"}, {"value": "Toxizitätsvergleichseinheit für Menschen (krebserregend) (HTP-c)", "lang": "de"}], "type": "LCIA method data set", "refObjectId": "2299222a-bbd8-474f-9d4f-4dd1f18aea7c", "uri": "../lciamethods/2299222a-bbd8-474f-9d4f-4dd1f18aea7c.xml"}, "other": {"anies": [{"name": "referenceToUnitGroupDataSet", "value": {"shortDescription": [{"value": "CTUh", "lang": "en"}], "type": "unit group data set", "refObjectId": "d4c9523e-2d7e-49fd-8469-998f547d3a70", "uri": "../unitgroups/d4c9523e-2d7e-49fd-8469-998f547d3a70.xml"}}, {"value": "4.00090422420216E-09", "module": "A1-A3"}, {"value": "9.44961375681E-11", "module": "A4"}, {"value": "1.28095769195644E-12", "module": "A5"}, {"value": "0", "module": "C1"}, {"value": "1.85822139184677E-11", "module": "C2"}, {"value": "8.2424516663435E-11", "module": "C3"}, {"value": "1.02214712348933E-11", "module": "C4"}, {"value": "-6.45663729883133E-10", "module": "D"}]}}, {"referenceToLCIAMethodDataSet": {"shortDescription": [{"value": "Comparative toxic unit for humans (noncarcinogenic) (HTP-nc)", "lang": "en"}, {"value": "Toxizitätsvergleichseinheit für Menschen (nicht krebserregend) (HTP-nc)", "lang": "de"}], "type": "LCIA method data set", "refObjectId": "3af763a5-b7a1-48c9-9cee-1f223481fcef", "uri": "../lciamethods/3af763a5-b7a1-48c9-9cee-1f223481fcef.xml"}, "other": {"anies": [{"name": "referenceToUnitGroupDataSet", "value": {"shortDescription": [{"value": "CTUh", "lang": "en"}], "type": "unit group data set", "refObjectId": "d4c9523e-2d7e-49fd-8469-998f547d3a70", "uri": "../unitgroups/d4c9523e-2d7e-49fd-8469-998f547d3a70.xml"}}, {"value": "1.43652082912536E-07", "module": "A1-A3"}, {"value": "4.17343769475958E-09", "module": "A4"}, {"value": "1.06820471758395E-11", "module": "A5"}, {"value": "0", "module": "C1"}, {"value": "8.20686580586753E-10", "module": "C2"}, {"value": "1.25291846728082E-09", "module": "C3"}, {"value": "1.07924122952572E-09", "module": "C4"}, {"value": "-1.59272824673904E-08", "module": "D"}]}}, {"referenceToLCIAMethodDataSet": {"shortDescription": [{"value": "Soil quality index (SQP)", "lang": "en"}, {"value": "Bodenqualitätsindex (SQP)", "lang": "de"}], "type": "LCIA method data set", "refObjectId": "b2ad6890-c78d-11e6-9d9d-cec0c932ce01", "uri": "../lciamethods/b2ad6890-c78d-11e6-9d9d-cec0c932ce01.xml"}, "other": {"anies": [{"name": "referenceToUnitGroupDataSet", "value": {"shortDescription": [{"value": "SQP", "lang": "en"}], "type": "unit group data set", "refObjectId": "f130951c-e67f-4f7f-8dd4-665de3974e18", "uri": "../unitgroups/f130951c-e67f-4f7f-8dd4-665de3974e18.xml"}}, {"value": "45.8487602392907", "module": "A1-A3"}, {"value": "2.77752049940212", "module": "A4"}, {"value": "0.00771171180728012", "module": "A5"}, {"value": "0", "module": "C1"}, {"value": "0.546186134281148", "module": "C2"}, {"value": "1.14022965664255", "module": "C3"}, {"value": "0.0295578563620756", "module": "C4"}, {"value": "-11.1726535127981", "module": "D"}]}}]}, "otherAttributes": {"{http://www.indata.network/EPD/2019}epd-version": "1.2"}, "version": "1.1", "locations": "../ILCDLocations.xml"}