{"processInformation": {"dataSetInformation": {"UUID": "ceffefa2-299b-49d8-b9a6-4f759a546271", "name": {"baseName": [{"value": "FFB-VS", "lang": "de"}, {"value": "FFB-VS", "lang": "en"}], "functionalUnitFlowProperties": [{"lang": "de"}]}, "classificationInformation": {"classification": [{"class": [{"value": "Dämmstoffe", "level": 0, "classId": "2"}, {"value": "Mineralwolle", "level": 1, "classId": "2.1"}, {"value": "Mineralwolle", "level": 2, "classId": "2.1.01"}], "name": "OEKOBAU.DAT"}, {"class": [{"value": "02 Bauprodukte", "level": 0}, {"value": "Brandschutz", "level": 1}, {"value": "Vorgeformte Brandschutzsysteme zur Kabel- und Rohrabschottung", "level": 2}], "name": "IBUCategories"}]}, "generalComment": [{"value": "Bei dem deklarierten Produkt handelt es sich um eine Steinwolle-Platte aus knstlichen, parallel zur Oberflche der Platten ausgerichteten Mineralfasern, die im Heiverfahren hergestellt und nach dem Auskhlen durch hinzugefgten Klebstoff zusammengehalten werden. Die Platten sind beidseitig mit einer durch Kunststoffasern verstrkten Aluminiumfolie kaschiert, die im heien Plattenzustand aufgebracht und mit dem Klebstoff, der die Mineralfasern zusammenhlt, fixiert wird. Ein Blhgraphit-Streifen (RSI-Streifen) wird mit einer bedruckten PVC-Klebefolie an einer Lngsseite befestigt.", "lang": "de"}, {"value": "The declared product is a mineral wool panel made of artificial mineral fibres running parallel to the surface which is manufactured in a procedure using heat and held together by added adhesive once cooled. The panels are clad on both sides with plastic fibre-reinforced aluminium foil which is applied whilst the panel is hot and fixed with the adhesive which holds the mineral fibres together. An expandable graphite strip (RSI strip) with a printed PVC adhesive foil is fixed to one longitudinal side.", "lang": "en"}], "other": {"anies": [{"scenario": [{"description": [{"value": "100% Deponierung (C1,C2,C3,C4/2,D)", "lang": "de"}, {"value": "waste incineration", "lang": "en"}], "name": "S1", "default": true}, {"description": [{"value": "NULL", "lang": "de"}, {"value": "disposal in landfill", "lang": "en"}], "name": "S2"}]}]}}, "quantitativeReference": {"referenceToReferenceFlow": [0]}, "time": {"referenceYear": 2024, "dataSetValidUntil": 2029, "other": {"anies": [{"name": "publicationDateOfEPD", "value": 1716422400000}]}}, "geography": {"locationOfOperationSupplyOrProduction": {"location": "RER"}}, "technology": {"technologyDescriptionAndIncludedProcesses": [{"value": "Bei dem deklarierten Produkt handelt es sich um einen Brandschutzriegel-Riegel aus künstlichen, parallel zur Oberfläche der Platten ausgerichteten Mineralfasern. Das Produkt wird im Heißverfahren hergestellt und nach dem Auskühlen durch hinzugefügten Klebstoff zusammengehalten. Die Platten sind beidseitig mit einer durch Glasfasern verstärkten Aluminiumfolie kaschiert. Ein Blähgraphit-Streifen wird mit einer bedruckten PVC-Klebefolie an einer Längsseite des zu deklarierenden Produkts befestigt. \nTechnische Daten: \nNachfolgend sind die bautechnischen Daten des im Rahmen der kobilanzstudie betrachteten, durchschnittlichen Produkts in tabellarischer Form dargestellt. \nDeklarierte Einheit: \nDie deklarierte Einheit ist 1 m Brandschutzriegel aus Mineralwolle mit einer glasfaserverstrkten Aluminiumfolie und einem Blhgraphit-Streifen.", "lang": "de"}, {"value": "Bei dem deklarierten Produkt handelt es sich um einen Brandschutzriegel aus künstlichen, parallel zur Oberfläche der Platten ausgerichteten Mineralfasern. Das Produkt wird im Heißverfahren hergestellt und nach dem Auskühlen durch hinzugefügten Klebstoff zusammengehalten. Die Platten sind beidseitig mit einer durch Glasfasern verstärkten Aluminiumfolie kaschiert. Ein Blähgraphit-Streifen wird mit einer bedruckten PVC-Klebefolie an einer Längsseite des zu deklarierenden Produkts befestigt. \nTechnical data: \nThe constructional data of the average product examined as part of the LCA study is shown in table form below. \nDeclared unit: \nThe declared unit is 1 m of mineral wool fire protection barrier with a glass fibre-reinforced aluminium foil and an expandable graphite strip.", "lang": "en"}], "technologicalApplicability": [{"value": "Bei dem zu deklarierenden Bauprodukt handelt es sich um einen horizontal verbauten Brandriegel in einer Gebudeverkleidung. FFB-VS wurde entwickelt, um einen 25- bzw. 50-mm-Lftungsspalt bereitzustellen, der den Luftstrom und die Feuchtigkeit an der Rckseite der Gebudeverkleidung (vorgehngte Fassade) passieren lsst und sich unter Brandbedingungen schliet. Bei Brand dehnt sich das Intumeszenzmittel entlang der Vorderkante horizontal aus, um den Spalt zu schlieen und den Durchgang von Feuer zu verhindern. Dadurch wird der \"Kamineffekt\" und damit die vertikale Brandausbreitung von unteren in darberliegende Stockwerke unterbunden.", "lang": "de"}, {"value": "The building product to be declared is a horizontally installed fire protection barrier built in building cladding. FFB-VS was developed to provide a 25 or 50 mm ventilation gap which lets through the airflow and moisture on the back of the building cladding (ventilated rainscreen faade) and closes under fire conditions. In case of fire the intumescent agent along the front edge expands horizontally to close the gap and prevent the passage of fire. This prevents the chimney effect and the vertical spread of fire into the floors above.", "lang": "en"}]}}, "modellingAndValidation": {"LCIMethodAndAllocation": {"typeOfDataSet": "EPD", "referenceToLCAMethodDetails": [{"shortDescription": [{"value": "Vorgeformte Brandschutzsysteme zur Kabel- und Rohrabschottung.pdf", "lang": "de"}], "type": "source data set", "refObjectId": "3b63cd69-24d1-4b90-9934-506240f6c449"}], "other": {"anies": [{"name": "subType", "value": "average dataset"}]}}, "dataSourcesTreatmentAndRepresentativeness": {"referenceToDataSource": [{"shortDescription": [{"value": "GaBi Database (all versions)", "lang": "de"}], "type": "source data set", "refObjectId": "28d74cc0-db8b-4d7e-bc44-5f6d56ce0c4a"}, {"shortDescription": [{"value": "Sphera MLC (fka GaBi) CUP 2023.02", "lang": "de"}], "type": "source data set", "refObjectId": "cb600d3b-e85a-42b3-b059-5591e2757fbb"}], "useAdviceForDataSet": [{"value": "Gültigkeitsbereich: \nBei dem zu deklarierenden Bauprodukt handelt es ich um einen horizontal in der Gebudeverkleidung verbauten Brandschutzriegel aus Mineralwolle mit der Produktbezeichnung FFB-VS. Die Fertigung des Produkts erfolgt in mehreren Schritten, die nacheinander in den folgenden Werken durchgefhrt werden: \n\n1. Werk in Finnland \nParoc Group Oy, Energiakuja 3,\nP.O. Box 240, FI-00181 Helsinki, Finnland. \n\n2. Werk in Polen\nKORFF ISOLMATIC Sp. z o.o., ul. Lotnicza\n12, Wojnarowice, PL 55-050 Sobtka\n\n3. Werk in Deutschland\nfischerwerke GmbH & Co. KG\nKlaus-Fischer-Strasse 1,\n72178 Waldachtal, Deutschland \nSystemgrenze: \nEs wurde die Systemgrenze \"Wiege bis Werkstor – mit Optionen\" gewhlt. Der Lebenszyklus ist entsprechend EN15804 modular gestaltet. Die der vorliegenden EPD zugrundeliegende kobilanz bercksichtigt das Produktstadium(A1–A3), das Entsorgungsstadium (C1–C4) sowie Vorteile und Belastungen auerhalb der Systemgrenze (Modul D). Die Module A1 (Rohstoffbereitstellung), A2 (Transport) und A3(Herstellung) werden in der Auswertung aggregiert als Modul A1–A3 dargestellt. Die Module umfassen im Einzelnen die im Schaubild dargestellten Prozesse.\n\n (oranger Rahmen = Systemgrenze, graue Rahmen = Modulgrenzen)", "lang": "de"}, {"value": "Scope: \nThe building product to be declared is a mineral wool fire protection barrier built horizontally into the building cladding with the product designation FFB-VS. The product is manufactured in several steps which are performed in sequence in the following production facilities:\n\n1. Site in Finland\nParoc Group Oy, Energiakuja 3,\nP.O. Box 240, FI-00181 Helsinki, Finnland.\n\n2. Site in Poland\nKORFF ISOLMATIC Sp. z o.o., ul. Lotnicza\n12, Wojnarowice, PL 55-050 Sobtka\n3. Site in Germany\nfischerwerke GmbH & Co. KG\nKlaus-Fischer-Strasse 1,\n72178 Waldachtal, Germany \nSystem boundary: \nThe cradle to factory gate - with options system boundary was selected. The lifecycle is modular in accordance with EN15804. The LCA on which this EPD is based includes the product stage (A1-A3), the disposal state (C1-C4) and benefits and impacts beyond the system boundary (Module D). Modules A1 (raw material provision), A2 (Transport) and A3 (manufacture) are shown aggregated in the assessment as Module A1-A3. The modules include the individual processes shown in the diagram.\n\n(orange frame = system boundary, grey frame = module boundaries)", "lang": "en"}], "other": {"anies": [{"name": "referenceToOriginalEPD", "value": {"shortDescription": {"value": "FFB-VS.pdf", "defaultValue": "FFB-VS.pdf", "lstrings": [{"lang": "de", "value": "FFB-VS.pdf"}]}, "type": "source data set", "uuid": {"uuid": "6d5bb278-2f69-4f3c-b393-07cc58abdab1"}, "refObjectId": "6d5bb278-2f69-4f3c-b393-07cc58abdab1", "resourceURLs": ["https://oekobaudat.de/OEKOBAU.DAT/resource/sources/6d5bb278-2f69-4f3c-b393-07cc58abdab1/FFB-VS_18184.pdf?version=00.01.000"]}}]}}, "validation": {"review": [{"referenceToNameOfReviewerAndInstitution": [{"shortDescription": [{"value": "Institut Bauen und Umwelt e. V.", "lang": "de"}], "type": "contact data set", "refObjectId": "d111dbec-b024-4be5-86c5-752d6eb2cf95", "uri": "../contacts/d111dbec-b024-4be5-86c5-752d6eb2cf95.xml"}], "type": "Accredited third party review"}]}, "complianceDeclarations": {"compliance": [{"referenceToComplianceSystem": {"shortDescription": [{"value": "DIN EN 15804+A2", "lang": "de"}], "type": "source data set", "refObjectId": "c0016b33-8cf7-415c-ac6e-deba0d21440d", "uri": "../sources/c0016b33-8cf7-415c-ac6e-deba0d21440d.xml"}}, {"referenceToComplianceSystem": {"shortDescription": [{"value": "ISO 14025", "lang": "de"}], "type": "source data set", "refObjectId": "4f2eb655-6e44-4874-a95a-e28f5442cd4d", "uri": "../sources/4f2eb655-6e44-4874-a95a-e28f5442cd4d.xml"}}]}}, "administrativeInformation": {"commissionerAndGoal": {"referenceToCommissioner": [{"shortDescription": [{"value": "fischerwerke GmbH & Co. KG", "lang": "de"}], "type": "contact data set", "refObjectId": "75f1ded5-92d7-4664-9417-67a5933d1795", "uri": "../contacts/75f1ded5-92d7-4664-9417-67a5933d1795.xml"}]}, "dataGenerator": {"referenceToPersonOrEntityGeneratingTheDataSet": [{"shortDescription": [{"value": "SKZ - Das Kunststoff-Zentrum", "lang": "de"}], "type": "contact data set", "refObjectId": "2da43b2d-777d-45c6-ba4b-76c55a616a00", "uri": "../contacts/2da43b2d-777d-45c6-ba4b-76c55a616a00.xml"}]}, "dataEntryBy": {"timeStamp": 1716422400000, "referenceToDataSetFormat": [{"shortDescription": [{"value": "ILCD Format", "lang": "de"}], "type": "source data set", "refObjectId": "a97a0155-0234-4b87-b4ce-a45da52f2a40", "uri": "../sources/a97a0155-0234-4b87-b4ce-a45da52f2a40.xml"}, {"shortDescription": [{"value": "EPD-Datenformaterweiterungen v1.2", "lang": "de"}, {"value": "EPD Data Format Extensions v1.2", "lang": "en"}], "type": "source data set", "refObjectId": "a29449fd-aa2f-4de8-b5d7-4b06b43c6fde", "uri": "../sources/a29449fd-aa2f-4de8-b5d7-4b06b43c6fde.xml"}]}, "publicationAndOwnership": {"dataSetVersion": "00.04.000", "referenceToRegistrationAuthority": {"shortDescription": [{"value": "Institut Bauen und Umwelt e. V.", "lang": "de"}], "type": "contact data set", "refObjectId": "d111dbec-b024-4be5-86c5-752d6eb2cf95", "uri": "../contacts/d111dbec-b024-4be5-86c5-752d6eb2cf95.xml"}, "registrationNumber": "EPD-FIW-20230532-CBA1-DE", "referenceToOwnershipOfDataSet": {"shortDescription": [{"value": "fischerwerke GmbH & Co. KG", "lang": "de"}], "type": "contact data set", "refObjectId": "75f1ded5-92d7-4664-9417-67a5933d1795", "uri": "../contacts/75f1ded5-92d7-4664-9417-67a5933d1795.xml"}, "copyright": true, "licenseType": "Free of charge for all users and uses", "accessRestrictions": [{"value": "None", "lang": "en"}], "other": {"anies": [{"name": "referenceToPublisher", "value": {"shortDescription": [{"value": "Institut Bauen und Umwelt e. V.", "lang": "de"}], "type": "contact data set", "refObjectId": "d111dbec-b024-4be5-86c5-752d6eb2cf95", "uri": "../contacts/d111dbec-b024-4be5-86c5-752d6eb2cf95.xml"}}]}}}, "exchanges": {"exchange": [{"dataSetInternalID": 0, "referenceToFlowDataSet": {"shortDescription": [{"value": "Brandschutzriegel FFB-VS (Brandschutzriegel FFB-VS)", "lang": "de"}], "type": "flow data set", "refObjectId": "a6135340-6d09-0d08-6113-0e52772cd5df", "uri": "../flows/a6135340-6d09-0d08-6113-0e52772cd5df.xml"}, "meanAmount": 1.0, "referencesToDataSource": {}, "referenceFlow": true, "resolvedFlowVersion": "00.04.000", "resultingflowAmount": 1.0, "flowProperties": [{"name": [{"lang": "en", "value": "Volume"}, {"lang": "de", "value": "Volumen"}], "uuid": "93a60a56-a3c8-22da-a746-0800200c9a66", "referenceFlowProperty": true, "meanValue": 1.0, "referenceUnit": "m3", "unitGroupUUID": "cd950537-0a98-4044-9ba7-9f9a68d0a504"}], "materialProperties": [{"name": "gross density", "value": "90.0", "unit": "kg/m^3", "unitDescription": "kilograms per cubic metre"}], "typeOfFlow": "Product flow", "classification": {"classHierarchy": "Dämmstoffe / Mineralwolle / Mineralwolle", "name": "OEKOBAU.DAT"}}, {"dataSetInternalID": 1, "referenceToFlowDataSet": {"shortDescription": [{"value": "Erneuerbare Primärenergie als Energieträger (PERE)", "lang": "de"}, {"value": "Renewable primary energy as energy carrier (PERE)", "lang": "en"}], "type": "flow data set", "refObjectId": "20f32be5-0398-4288-9b6d-accddd195317", "uri": "../flows/20f32be5-0398-4288-9b6d-accddd195317.xml"}, "exchange direction": "INPUT", "other": {"anies": [{"name": "referenceToUnitGroupDataSet", "value": {"shortDescription": [{"value": "MJ", "lang": "de"}], "type": "unit group data set", "refObjectId": "93a60a57-a3c8-11da-a746-0800200c9a66", "uri": "../unitgroups/93a60a57-a3c8-11da-a746-0800200c9a66.xml"}}, {"value": "778.184010340589", "module": "A1-A3"}, {"value": "0", "module": "C1"}, {"value": "0.463714293538407", "module": "C2"}, {"value": "0", "module": "C3"}, {"value": "61.5999560399348", "module": "C4", "scenario": "S1"}, {"value": "3.53108798304208", "module": "C4", "scenario": "S2"}, {"value": "0", "module": "D"}]}, "resolvedFlowVersion": "38.00.000", "flowProperties": [], "typeOfFlow": "Other flow", "classification": {"classHierarchy": "Quantities", "name": "GaBiCategories"}}, {"dataSetInternalID": 2, "referenceToFlowDataSet": {"shortDescription": [{"value": "Erneuerbare Primärenergie zur stofflichen Nutzung (PERM)", "lang": "de"}, {"value": "Renewable primary energy resources as material utilization (PERM)", "lang": "en"}], "type": "flow data set", "refObjectId": "fb3ec0de-548d-4508-aea5-00b73bf6f702", "uri": "../flows/fb3ec0de-548d-4508-aea5-00b73bf6f702.xml"}, "exchange direction": "INPUT", "other": {"anies": [{"name": "referenceToUnitGroupDataSet", "value": {"shortDescription": [{"value": "MJ", "lang": "de"}], "type": "unit group data set", "refObjectId": "93a60a57-a3c8-11da-a746-0800200c9a66", "uri": "../unitgroups/93a60a57-a3c8-11da-a746-0800200c9a66.xml"}}, {"value": "187.898592", "module": "A1-A3"}, {"value": "0", "module": "C1"}, {"value": "0", "module": "C2"}, {"value": "0", "module": "C3"}, {"value": "-0.992", "module": "C4", "scenario": "S1"}, {"value": "0", "module": "C4", "scenario": "S2"}, {"value": "0", "module": "D"}]}, "resolvedFlowVersion": "38.00.000", "flowProperties": [], "typeOfFlow": "Other flow", "classification": {"classHierarchy": "Quantities", "name": "GaBiCategories"}}, {"dataSetInternalID": 3, "referenceToFlowDataSet": {"shortDescription": [{"value": "Total erneuerbare Primärenergie (PERT)", "lang": "de"}, {"value": "Total use of renewable primary energy resources (PERT)", "lang": "en"}], "type": "flow data set", "refObjectId": "53f97275-fa8a-4cdd-9024-65936002acd0", "uri": "../flows/53f97275-fa8a-4cdd-9024-65936002acd0.xml"}, "exchange direction": "INPUT", "other": {"anies": [{"name": "referenceToUnitGroupDataSet", "value": {"shortDescription": [{"value": "MJ", "lang": "de"}], "type": "unit group data set", "refObjectId": "93a60a57-a3c8-11da-a746-0800200c9a66", "uri": "../unitgroups/93a60a57-a3c8-11da-a746-0800200c9a66.xml"}}, {"value": "966.082602340589", "module": "A1-A3"}, {"value": "0", "module": "C1"}, {"value": "0.463714293538407", "module": "C2"}, {"value": "0", "module": "C3"}, {"value": "60.6079560399348", "module": "C4", "scenario": "S1"}, {"value": "3.53108798304208", "module": "C4", "scenario": "S2"}, {"value": "0", "module": "D"}]}, "resolvedFlowVersion": "38.00.000", "flowProperties": [], "typeOfFlow": "Other flow", "classification": {"classHierarchy": "Quantities / Environmental quantities / EPD EN 15804 / LCI indicators", "name": "GaBiCategories"}}, {"dataSetInternalID": 4, "referenceToFlowDataSet": {"shortDescription": [{"value": "Nicht-erneuerbare Primärenergie als Energieträger (PENRE)", "lang": "de"}, {"value": "Non renewable primary energy as energy carrier (PENRE)", "lang": "en"}], "type": "flow data set", "refObjectId": "ac857178-2b45-46ec-892a-a9a4332f0372", "uri": "../flows/ac857178-2b45-46ec-892a-a9a4332f0372.xml"}, "exchange direction": "INPUT", "other": {"anies": [{"name": "referenceToUnitGroupDataSet", "value": {"shortDescription": [{"value": "MJ", "lang": "de"}], "type": "unit group data set", "refObjectId": "93a60a57-a3c8-11da-a746-0800200c9a66", "uri": "../unitgroups/93a60a57-a3c8-11da-a746-0800200c9a66.xml"}}, {"value": "1961.89453741341", "module": "A1-A3"}, {"value": "0", "module": "C1"}, {"value": "6.39603524346728", "module": "C2"}, {"value": "0", "module": "C3"}, {"value": "194.81820724296", "module": "C4", "scenario": "S1"}, {"value": "21.6823711704728", "module": "C4", "scenario": "S2"}, {"value": "0", "module": "D"}]}, "resolvedFlowVersion": "38.00.000", "flowProperties": [], "typeOfFlow": "Other flow", "classification": {"classHierarchy": "Quantities", "name": "GaBiCategories"}}, {"dataSetInternalID": 5, "referenceToFlowDataSet": {"shortDescription": [{"value": "Nicht-erneuerbare Primärenergie zur stofflichen Nutzung (PENRM)", "lang": "de"}, {"value": "Non renewable primary energy as material utilization (PENRM)", "lang": "en"}], "type": "flow data set", "refObjectId": "1421caa0-679d-4bf4-b282-0eb850ccae27", "uri": "../flows/1421caa0-679d-4bf4-b282-0eb850ccae27.xml"}, "exchange direction": "INPUT", "other": {"anies": [{"name": "referenceToUnitGroupDataSet", "value": {"shortDescription": [{"value": "MJ", "lang": "de"}], "type": "unit group data set", "refObjectId": "93a60a57-a3c8-11da-a746-0800200c9a66", "uri": "../unitgroups/93a60a57-a3c8-11da-a746-0800200c9a66.xml"}}, {"value": "36.83012", "module": "A1-A3"}, {"value": "0", "module": "C1"}, {"value": "0", "module": "C2"}, {"value": "0", "module": "C3"}, {"value": "-31.326", "module": "C4", "scenario": "S1"}, {"value": "0", "module": "C4", "scenario": "S2"}, {"value": "0", "module": "D"}]}, "resolvedFlowVersion": "38.00.000", "flowProperties": [], "typeOfFlow": "Other flow", "classification": {"classHierarchy": "Quantities", "name": "GaBiCategories"}}, {"dataSetInternalID": 6, "referenceToFlowDataSet": {"shortDescription": [{"value": "Total nicht erneuerbare Primärenergie (PENRT)", "lang": "de"}, {"value": "Total use of non renewable primary energy resources (PENRT)", "lang": "en"}], "type": "flow data set", "refObjectId": "06159210-646b-4c8d-8583-da9b3b95a6c1", "uri": "../flows/06159210-646b-4c8d-8583-da9b3b95a6c1.xml"}, "exchange direction": "INPUT", "other": {"anies": [{"name": "referenceToUnitGroupDataSet", "value": {"shortDescription": [{"value": "MJ", "lang": "de"}], "type": "unit group data set", "refObjectId": "93a60a57-a3c8-11da-a746-0800200c9a66", "uri": "../unitgroups/93a60a57-a3c8-11da-a746-0800200c9a66.xml"}}, {"value": "1998.72465741341", "module": "A1-A3"}, {"value": "0", "module": "C1"}, {"value": "6.39603524346728", "module": "C2"}, {"value": "0", "module": "C3"}, {"value": "163.49220724296", "module": "C4", "scenario": "S1"}, {"value": "21.6823711704728", "module": "C4", "scenario": "S2"}, {"value": "0", "module": "D"}]}, "resolvedFlowVersion": "38.00.000", "flowProperties": [], "typeOfFlow": "Other flow", "classification": {"classHierarchy": "Quantities / Environmental quantities / EPD EN 15804 / LCI indicators", "name": "GaBiCategories"}}, {"dataSetInternalID": 7, "referenceToFlowDataSet": {"shortDescription": [{"value": "Einsatz von Sekundärstoffen (SM)", "lang": "de"}, {"value": "Use of secondary material (SM)", "lang": "en"}], "type": "flow data set", "refObjectId": "c6a1f35f-2d09-4f54-8dfb-97e502e1ce92", "uri": "../flows/c6a1f35f-2d09-4f54-8dfb-97e502e1ce92.xml"}, "exchange direction": "INPUT", "other": {"anies": [{"name": "referenceToUnitGroupDataSet", "value": {"shortDescription": [{"value": "kg", "lang": "de"}], "type": "unit group data set", "refObjectId": "ad38d542-3fe9-439d-9b95-2f5f7752acaf", "uri": "../unitgroups/ad38d542-3fe9-439d-9b95-2f5f7752acaf.xml"}}, {"value": "43.589547", "module": "A1-A3"}, {"value": "0", "module": "C1"}, {"value": "0", "module": "C2"}, {"value": "0", "module": "C3"}, {"value": "0", "module": "C4", "scenario": "S1"}, {"value": "0", "module": "C4", "scenario": "S2"}, {"value": "0", "module": "D"}]}, "resolvedFlowVersion": "38.00.000", "flowProperties": [], "typeOfFlow": "Other flow", "classification": {"classHierarchy": "Quantities / Environmental quantities / EPD EN 15804 / LCI indicators", "name": "GaBiCategories"}}, {"dataSetInternalID": 8, "referenceToFlowDataSet": {"shortDescription": [{"value": "Erneuerbare Sekundärbrennstoffe (RSF)", "lang": "de"}, {"value": "Use of renewable secondary fuels (RSF)", "lang": "en"}], "type": "flow data set", "refObjectId": "64333088-a55f-4aa2-9a31-c10b07816787", "uri": "../flows/64333088-a55f-4aa2-9a31-c10b07816787.xml"}, "exchange direction": "INPUT", "other": {"anies": [{"name": "referenceToUnitGroupDataSet", "value": {"shortDescription": [{"value": "MJ", "lang": "de"}], "type": "unit group data set", "refObjectId": "93a60a57-a3c8-11da-a746-0800200c9a66", "uri": "../unitgroups/93a60a57-a3c8-11da-a746-0800200c9a66.xml"}}, {"value": "0", "module": "A1-A3"}, {"value": "0", "module": "C1"}, {"value": "0", "module": "C2"}, {"value": "0", "module": "C3"}, {"value": "0", "module": "C4", "scenario": "S1"}, {"value": "0", "module": "C4", "scenario": "S2"}, {"value": "0", "module": "D"}]}, "resolvedFlowVersion": "38.00.000", "flowProperties": [], "typeOfFlow": "Other flow", "classification": {"classHierarchy": "Quantities / Environmental quantities / EPD EN 15804 / LCI indicators", "name": "GaBiCategories"}}, {"dataSetInternalID": 9, "referenceToFlowDataSet": {"shortDescription": [{"value": "Nicht erneuerbare Sekundärbrennstoffe (NRSF)", "lang": "de"}, {"value": "Use of non renewable secondary fuels (NRSF)", "lang": "en"}], "type": "flow data set", "refObjectId": "89def144-d39a-4287-b86f-efde453ddcb2", "uri": "../flows/89def144-d39a-4287-b86f-efde453ddcb2.xml"}, "exchange direction": "INPUT", "other": {"anies": [{"name": "referenceToUnitGroupDataSet", "value": {"shortDescription": [{"value": "MJ", "lang": "de"}], "type": "unit group data set", "refObjectId": "93a60a57-a3c8-11da-a746-0800200c9a66", "uri": "../unitgroups/93a60a57-a3c8-11da-a746-0800200c9a66.xml"}}, {"value": "0", "module": "A1-A3"}, {"value": "0", "module": "C1"}, {"value": "0", "module": "C2"}, {"value": "0", "module": "C3"}, {"value": "0", "module": "C4", "scenario": "S1"}, {"value": "0", "module": "C4", "scenario": "S2"}, {"value": "0", "module": "D"}]}, "resolvedFlowVersion": "38.00.000", "flowProperties": [], "typeOfFlow": "Other flow", "classification": {"classHierarchy": "Quantities / Environmental quantities / EPD EN 15804 / LCI indicators", "name": "GaBiCategories"}}, {"dataSetInternalID": 10, "referenceToFlowDataSet": {"shortDescription": [{"value": "Einsatz von Süßwasserressourcen (FW)", "lang": "de"}, {"value": "Use of net fresh water (FW)", "lang": "en"}], "type": "flow data set", "refObjectId": "3cf952c8-f3a4-461d-8c96-96456ca62246", "uri": "../flows/3cf952c8-f3a4-461d-8c96-96456ca62246.xml"}, "exchange direction": "INPUT", "other": {"anies": [{"name": "referenceToUnitGroupDataSet", "value": {"shortDescription": [{"value": "m^3", "lang": "de"}], "type": "unit group data set", "refObjectId": "cd950537-0a98-4044-9ba7-9f9a68d0a504", "uri": "../unitgroups/cd950537-0a98-4044-9ba7-9f9a68d0a504.xml"}}, {"value": "0.525950592337438", "module": "A1-A3"}, {"value": "0", "module": "C1"}, {"value": "0.000507892130384945", "module": "C2"}, {"value": "0", "module": "C3"}, {"value": "0.330231830184807", "module": "C4", "scenario": "S1"}, {"value": "0.00547374144907298", "module": "C4", "scenario": "S2"}, {"value": "0", "module": "D"}]}, "resolvedFlowVersion": "38.00.000", "flowProperties": [], "typeOfFlow": "Other flow", "classification": {"classHierarchy": "Quantities / Environmental quantities / EPD EN 15804 / LCI indicators", "name": "GaBiCategories"}}, {"dataSetInternalID": 11, "referenceToFlowDataSet": {"shortDescription": [{"value": "Gefährlicher Abfall zur Deponie (HWD)", "lang": "de"}, {"value": "Hazardous waste disposed (HWD)", "lang": "en"}], "type": "flow data set", "refObjectId": "430f9e0f-59b2-46a0-8e0d-55e0e84948fc", "uri": "../flows/430f9e0f-59b2-46a0-8e0d-55e0e84948fc.xml"}, "exchange direction": "OUTPUT", "other": {"anies": [{"name": "referenceToUnitGroupDataSet", "value": {"shortDescription": [{"value": "kg", "lang": "de"}], "type": "unit group data set", "refObjectId": "ad38d542-3fe9-439d-9b95-2f5f7752acaf", "uri": "../unitgroups/ad38d542-3fe9-439d-9b95-2f5f7752acaf.xml"}}, {"value": "1.95589292616263E-06", "module": "A1-A3"}, {"value": "0", "module": "C1"}, {"value": "1.98041549001624E-11", "module": "C2"}, {"value": "0", "module": "C3"}, {"value": "0", "module": "C4", "scenario": "S1"}, {"value": "4.71805030809692E-10", "module": "C4", "scenario": "S2"}, {"value": "0", "module": "D"}]}, "resolvedFlowVersion": "38.00.000", "flowProperties": [], "typeOfFlow": "Other flow", "classification": {"classHierarchy": "Quantities / Environmental quantities / EPD EN 15804 / LCI indicators", "name": "GaBiCategories"}}, {"dataSetInternalID": 12, "referenceToFlowDataSet": {"shortDescription": [{"value": "Entsorgter nicht gefährlicher Abfall (NHWD)", "lang": "de"}, {"value": "Non hazardous waste disposed (NHWD)", "lang": "en"}], "type": "flow data set", "refObjectId": "b29ef66b-e286-4afa-949f-62f1a7b4d7fa", "uri": "../flows/b29ef66b-e286-4afa-949f-62f1a7b4d7fa.xml"}, "exchange direction": "OUTPUT", "other": {"anies": [{"name": "referenceToUnitGroupDataSet", "value": {"shortDescription": [{"value": "kg", "lang": "de"}], "type": "unit group data set", "refObjectId": "ad38d542-3fe9-439d-9b95-2f5f7752acaf", "uri": "../unitgroups/ad38d542-3fe9-439d-9b95-2f5f7752acaf.xml"}}, {"value": "43.9279367730097", "module": "A1-A3"}, {"value": "0", "module": "C1"}, {"value": "0.000975006164583313", "module": "C2"}, {"value": "0", "module": "C3"}, {"value": "14.9688403107284", "module": "C4", "scenario": "S1"}, {"value": "108.412437527163", "module": "C4", "scenario": "S2"}, {"value": "0", "module": "D"}]}, "resolvedFlowVersion": "38.00.000", "flowProperties": [], "typeOfFlow": "Other flow", "classification": {"classHierarchy": "Quantities / Environmental quantities / EPD EN 15804 / LCI indicators", "name": "GaBiCategories"}}, {"dataSetInternalID": 13, "referenceToFlowDataSet": {"shortDescription": [{"value": "Entsorgter radioaktiver Abfall (RWD)", "lang": "de"}, {"value": "Radioactive waste disposed (RWD)", "lang": "en"}], "type": "flow data set", "refObjectId": "3449546e-52ad-4b39-b809-9fb77cea8ff6", "uri": "../flows/3449546e-52ad-4b39-b809-9fb77cea8ff6.xml"}, "exchange direction": "OUTPUT", "other": {"anies": [{"name": "referenceToUnitGroupDataSet", "value": {"shortDescription": [{"value": "kg", "lang": "de"}], "type": "unit group data set", "refObjectId": "ad38d542-3fe9-439d-9b95-2f5f7752acaf", "uri": "../unitgroups/ad38d542-3fe9-439d-9b95-2f5f7752acaf.xml"}}, {"value": "0.0725167523391245", "module": "A1-A3"}, {"value": "0", "module": "C1"}, {"value": "1.1969799532912E-05", "module": "C2"}, {"value": "0", "module": "C3"}, {"value": "0.0115170489333973", "module": "C4", "scenario": "S1"}, {"value": "0.000247207956107238", "module": "C4", "scenario": "S2"}, {"value": "0", "module": "D"}]}, "resolvedFlowVersion": "38.00.000", "flowProperties": [], "typeOfFlow": "Other flow", "classification": {"classHierarchy": "Quantities / Environmental quantities / EPD EN 15804 / LCI indicators", "name": "GaBiCategories"}}, {"dataSetInternalID": 14, "referenceToFlowDataSet": {"shortDescription": [{"value": "Komponenten für die Wiederverwendung (CRU)", "lang": "de"}, {"value": "Components for re-use (CRU)", "lang": "en"}], "type": "flow data set", "refObjectId": "a2b32f97-3fc7-4af2-b209-525bc6426f33", "uri": "../flows/a2b32f97-3fc7-4af2-b209-525bc6426f33.xml"}, "exchange direction": "OUTPUT", "other": {"anies": [{"name": "referenceToUnitGroupDataSet", "value": {"shortDescription": [{"value": "kg", "lang": "de"}], "type": "unit group data set", "refObjectId": "ad38d542-3fe9-439d-9b95-2f5f7752acaf", "uri": "../unitgroups/ad38d542-3fe9-439d-9b95-2f5f7752acaf.xml"}}, {"value": "0", "module": "A1-A3"}, {"value": "0", "module": "C1"}, {"value": "0", "module": "C2"}, {"value": "0", "module": "C3"}, {"value": "0", "module": "C4", "scenario": "S1"}, {"value": "0", "module": "C4", "scenario": "S2"}, {"value": "0", "module": "D"}]}, "resolvedFlowVersion": "38.00.000", "flowProperties": [], "typeOfFlow": "Other flow", "classification": {"classHierarchy": "Quantities / Environmental quantities / EPD EN 15804 / LCI indicators", "name": "GaBiCategories"}}, {"dataSetInternalID": 15, "referenceToFlowDataSet": {"shortDescription": [{"value": "Stoffe zum Recycling (MFR)", "lang": "de"}, {"value": "Materials for recycling (MFR)", "lang": "en"}], "type": "flow data set", "refObjectId": "d7fe48a5-4103-49c8-9aae-b0b5dfdbd6ae", "uri": "../flows/d7fe48a5-4103-49c8-9aae-b0b5dfdbd6ae.xml"}, "exchange direction": "OUTPUT", "other": {"anies": [{"name": "referenceToUnitGroupDataSet", "value": {"shortDescription": [{"value": "kg", "lang": "de"}], "type": "unit group data set", "refObjectId": "ad38d542-3fe9-439d-9b95-2f5f7752acaf", "uri": "../unitgroups/ad38d542-3fe9-439d-9b95-2f5f7752acaf.xml"}}, {"value": "0", "module": "A1-A3"}, {"value": "0", "module": "C1"}, {"value": "0", "module": "C2"}, {"value": "0", "module": "C3"}, {"value": "0", "module": "C4", "scenario": "S1"}, {"value": "0", "module": "C4", "scenario": "S2"}, {"value": "0", "module": "D"}]}, "resolvedFlowVersion": "38.00.000", "flowProperties": [], "typeOfFlow": "Other flow", "classification": {"classHierarchy": "Quantities / Environmental quantities / EPD EN 15804 / LCI indicators", "name": "GaBiCategories"}}, {"dataSetInternalID": 16, "referenceToFlowDataSet": {"shortDescription": [{"value": "Stoffe für die Energierückgewinnung (MER)", "lang": "de"}, {"value": "Materials for energy recovery (MER)", "lang": "en"}], "type": "flow data set", "refObjectId": "59a9181c-3aaf-46ee-8b13-2b3723b6e447", "uri": "../flows/59a9181c-3aaf-46ee-8b13-2b3723b6e447.xml"}, "exchange direction": "OUTPUT", "other": {"anies": [{"name": "referenceToUnitGroupDataSet", "value": {"shortDescription": [{"value": "kg", "lang": "de"}], "type": "unit group data set", "refObjectId": "ad38d542-3fe9-439d-9b95-2f5f7752acaf", "uri": "../unitgroups/ad38d542-3fe9-439d-9b95-2f5f7752acaf.xml"}}, {"value": "0", "module": "A1-A3"}, {"value": "0", "module": "C1"}, {"value": "0", "module": "C2"}, {"value": "0", "module": "C3"}, {"value": "0", "module": "C4", "scenario": "S1"}, {"value": "0", "module": "C4", "scenario": "S2"}, {"value": "0", "module": "D"}]}, "resolvedFlowVersion": "38.00.000", "flowProperties": [], "typeOfFlow": "Other flow", "classification": {"classHierarchy": "Quantities / Environmental quantities / EPD EN 15804 / LCI indicators", "name": "GaBiCategories"}}, {"dataSetInternalID": 17, "referenceToFlowDataSet": {"shortDescription": [{"value": "Exportierte elektrische Energie (EEE)", "lang": "de"}, {"value": "Exported electrical energy (EEE)", "lang": "en"}], "type": "flow data set", "refObjectId": "4da0c987-2b76-40d6-9e9e-82a017aaaf29", "uri": "../flows/4da0c987-2b76-40d6-9e9e-82a017aaaf29.xml"}, "exchange direction": "OUTPUT", "other": {"anies": [{"name": "referenceToUnitGroupDataSet", "value": {"shortDescription": [{"value": "MJ", "lang": "de"}], "type": "unit group data set", "refObjectId": "93a60a57-a3c8-11da-a746-0800200c9a66", "uri": "../unitgroups/93a60a57-a3c8-11da-a746-0800200c9a66.xml"}}, {"value": "8.87725554045713", "module": "A1-A3"}, {"value": "0", "module": "C1"}, {"value": "0", "module": "C2"}, {"value": "0", "module": "C3"}, {"value": "0", "module": "C4", "scenario": "S1"}, {"value": "0", "module": "C4", "scenario": "S2"}, {"value": "0", "module": "D"}]}, "resolvedFlowVersion": "38.00.000", "flowProperties": [], "typeOfFlow": "Other flow", "classification": {"classHierarchy": "Quantities / Environmental quantities / EPD EN 15804 / LCI indicators", "name": "GaBiCategories"}}, {"dataSetInternalID": 18, "referenceToFlowDataSet": {"shortDescription": [{"value": "Exportierte thermische Energie (EET)", "lang": "de"}, {"value": "Exported thermal energy (EET)", "lang": "en"}], "type": "flow data set", "refObjectId": "98daf38a-7a79-46d3-9a37-2b7bd0955810", "uri": "../flows/98daf38a-7a79-46d3-9a37-2b7bd0955810.xml"}, "exchange direction": "OUTPUT", "other": {"anies": [{"name": "referenceToUnitGroupDataSet", "value": {"shortDescription": [{"value": "MJ", "lang": "de"}], "type": "unit group data set", "refObjectId": "93a60a57-a3c8-11da-a746-0800200c9a66", "uri": "../unitgroups/93a60a57-a3c8-11da-a746-0800200c9a66.xml"}}, {"value": "4.50882979330505", "module": "A1-A3"}, {"value": "0", "module": "C1"}, {"value": "0", "module": "C2"}, {"value": "0", "module": "C3"}, {"value": "0", "module": "C4", "scenario": "S1"}, {"value": "0", "module": "C4", "scenario": "S2"}, {"value": "0", "module": "D"}]}, "resolvedFlowVersion": "38.00.000", "flowProperties": [], "typeOfFlow": "Other flow", "classification": {"classHierarchy": "Quantities / Environmental quantities / EPD EN 15804 / LCI indicators", "name": "GaBiCategories"}}]}, "LCIAResults": {"LCIAResult": [{"referenceToLCIAMethodDataSet": {"shortDescription": [{"value": "Globales Erwärmungspotenzial total (GWP-total)", "lang": "de"}, {"value": "Global Warming Potential total (GWP-total)", "lang": "en"}], "type": "LCIA method data set", "refObjectId": "6a37f984-a4b3-458a-a20a-64418c145fa2", "uri": "../lciamethods/6a37f984-a4b3-458a-a20a-64418c145fa2.xml"}, "other": {"anies": [{"name": "referenceToUnitGroupDataSet", "value": {"shortDescription": [{"value": "kg CO_(2)-Äq.", "lang": "de"}], "type": "unit group data set", "refObjectId": "1ebf3012-d0db-4de2-aefd-ef30cedb0be1", "uri": "../unitgroups/1ebf3012-d0db-4de2-aefd-ef30cedb0be1.xml"}}, {"value": "145.384750203006", "module": "A1-A3"}, {"value": "0", "module": "C1"}, {"value": "0.47430066246014", "module": "C2"}, {"value": "0", "module": "C3"}, {"value": "15.7312167671387", "module": "C4", "scenario": "S1"}, {"value": "1.60848647991856", "module": "C4", "scenario": "S2"}, {"value": "0", "module": "D"}]}}, {"referenceToLCIAMethodDataSet": {"shortDescription": [{"value": "Globales Erwärmungspotenzial fossil (GWP-fossil)", "lang": "de"}, {"value": "Global Warming Potential fossil fuels (GWP-fossil)", "lang": "en"}], "type": "LCIA method data set", "refObjectId": "5f635281-343e-44fb-83df-1971b155e6b6", "uri": "../lciamethods/5f635281-343e-44fb-83df-1971b155e6b6.xml"}, "other": {"anies": [{"name": "referenceToUnitGroupDataSet", "value": {"shortDescription": [{"value": "kg CO_(2)-Äq.", "lang": "de"}], "type": "unit group data set", "refObjectId": "1ebf3012-d0db-4de2-aefd-ef30cedb0be1", "uri": "../unitgroups/1ebf3012-d0db-4de2-aefd-ef30cedb0be1.xml"}}, {"value": "145.100978907456", "module": "A1-A3"}, {"value": "0", "module": "C1"}, {"value": "0.469968619495454", "module": "C2"}, {"value": "0", "module": "C3"}, {"value": "15.6635020925342", "module": "C4", "scenario": "S1"}, {"value": "1.60343165896084", "module": "C4", "scenario": "S2"}, {"value": "0", "module": "D"}]}}, {"referenceToLCIAMethodDataSet": {"shortDescription": [{"value": "Globales Erwärmungspotenzial biogen (GWP-biogenic)", "lang": "de"}, {"value": "Global Warming Potential biogenic (GWP-biogenic)", "lang": "en"}], "type": "LCIA method data set", "refObjectId": "2356e1ab-0185-4db5-86e5-16de51c7485c", "uri": "../lciamethods/2356e1ab-0185-4db5-86e5-16de51c7485c.xml"}, "other": {"anies": [{"name": "referenceToUnitGroupDataSet", "value": {"shortDescription": [{"value": "kg CO_(2)-Äq.", "lang": "de"}], "type": "unit group data set", "refObjectId": "1ebf3012-d0db-4de2-aefd-ef30cedb0be1", "uri": "../unitgroups/1ebf3012-d0db-4de2-aefd-ef30cedb0be1.xml"}}, {"value": "0.0318299568545441", "module": "A1-A3"}, {"value": "0", "module": "C1"}, {"value": "0", "module": "C2"}, {"value": "0", "module": "C3"}, {"value": "0.0598225653680522", "module": "C4", "scenario": "S1"}, {"value": "0", "module": "C4", "scenario": "S2"}, {"value": "0", "module": "D"}]}}, {"referenceToLCIAMethodDataSet": {"shortDescription": [{"value": "Globales Erwärmungspotenzial luluc (GWP-luluc)", "lang": "de"}, {"value": "Global Warming Potential luluc (GWP-luluc)", "lang": "en"}], "type": "LCIA method data set", "refObjectId": "4331bbdb-978a-490d-8707-eeb047f01a55", "uri": "../lciamethods/4331bbdb-978a-490d-8707-eeb047f01a55.xml"}, "other": {"anies": [{"name": "referenceToUnitGroupDataSet", "value": {"shortDescription": [{"value": "kg CO_(2)-Äq.", "lang": "de"}], "type": "unit group data set", "refObjectId": "1ebf3012-d0db-4de2-aefd-ef30cedb0be1", "uri": "../unitgroups/1ebf3012-d0db-4de2-aefd-ef30cedb0be1.xml"}}, {"value": "0.25194133869498", "module": "A1-A3"}, {"value": "0", "module": "C1"}, {"value": "0.00433204296468648", "module": "C2"}, {"value": "0", "module": "C3"}, {"value": "0.00789210923644151", "module": "C4", "scenario": "S1"}, {"value": "0.00505482095771617", "module": "C4", "scenario": "S2"}, {"value": "0", "module": "D"}]}}, {"referenceToLCIAMethodDataSet": {"shortDescription": [{"value": "Abbau Potential der stratosphärischen Ozonschicht (ODP)", "lang": "de"}, {"value": "Depletion potential of the stratospheric ozone layer (ODP)", "lang": "en"}], "type": "LCIA method data set", "refObjectId": "b5c629d6-def3-11e6-bf01-fe55135034f3", "uri": "../lciamethods/b5c629d6-def3-11e6-bf01-fe55135034f3.xml"}, "other": {"anies": [{"name": "referenceToUnitGroupDataSet", "value": {"shortDescription": [{"value": "kg CFC11-Äq.", "lang": "de"}], "type": "unit group data set", "refObjectId": "d9e957c9-7309-4474-bf3a-7777df6c4e5b", "uri": "../unitgroups/d9e957c9-7309-4474-bf3a-7777df6c4e5b.xml"}}, {"value": "3.54722055630827E-10", "module": "A1-A3"}, {"value": "0", "module": "C1"}, {"value": "6.08623041227069E-14", "module": "C2"}, {"value": "0", "module": "C3"}, {"value": "1.03391384558251E-10", "module": "C4", "scenario": "S1"}, {"value": "4.13836196187573E-12", "module": "C4", "scenario": "S2"}, {"value": "0", "module": "D"}]}}, {"referenceToLCIAMethodDataSet": {"shortDescription": [{"value": "Versauerungspotenzial von Boden und Wasser (AP)", "lang": "de"}, {"value": "Acidification potential of land and water (AP)", "lang": "en"}], "type": "LCIA method data set", "refObjectId": "b5c611c6-def3-11e6-bf01-fe55135034f3", "uri": "../lciamethods/b5c611c6-def3-11e6-bf01-fe55135034f3.xml"}, "other": {"anies": [{"name": "referenceToUnitGroupDataSet", "value": {"shortDescription": [{"value": "mol H^(+)-Äq.", "lang": "de"}], "type": "unit group data set", "refObjectId": "42e089ac-92bf-4bf2-8ca1-5fc40d18f2ed", "uri": "../unitgroups/42e089ac-92bf-4bf2-8ca1-5fc40d18f2ed.xml"}}, {"value": "1.0416211657135", "module": "A1-A3"}, {"value": "0", "module": "C1"}, {"value": "0.000788165758193714", "module": "C2"}, {"value": "0", "module": "C3"}, {"value": "0.0276049939927143", "module": "C4", "scenario": "S1"}, {"value": "0.0115396320601202", "module": "C4", "scenario": "S2"}, {"value": "0", "module": "D"}]}}, {"referenceToLCIAMethodDataSet": {"shortDescription": [{"value": "Eutrophierungspotenzial Süßwasser (EP-freshwater)", "lang": "de"}, {"value": "Eutrophication potential aquatic freshwater (EP-freshwater)", "lang": "en"}], "type": "LCIA method data set", "refObjectId": "b53ec18f-7377-4ad3-86eb-cc3f4f276b2b", "uri": "../lciamethods/b53ec18f-7377-4ad3-86eb-cc3f4f276b2b.xml"}, "other": {"anies": [{"name": "referenceToUnitGroupDataSet", "value": {"shortDescription": [{"value": "kg P-Äq.", "lang": "de"}], "type": "unit group data set", "refObjectId": "0429039d-a61d-4590-ba67-aa4a20a810a1", "uri": "../unitgroups/0429039d-a61d-4590-ba67-aa4a20a810a1.xml"}}, {"value": "0.000320434519056613", "module": "A1-A3"}, {"value": "0", "module": "C1"}, {"value": "1.71014674475116E-06", "module": "C2"}, {"value": "0", "module": "C3"}, {"value": "4.84113738847391E-05", "module": "C4", "scenario": "S1"}, {"value": "3.27629641753098E-06", "module": "C4", "scenario": "S2"}, {"value": "0", "module": "D"}]}}, {"referenceToLCIAMethodDataSet": {"shortDescription": [{"value": "Eutrophierungspotenzial Salzwasser (EP-marine)", "lang": "de"}, {"value": "Eutrophication potential aquatic marine (EP-marine)", "lang": "en"}], "type": "LCIA method data set", "refObjectId": "b5c619fa-def3-11e6-bf01-fe55135034f3", "uri": "../lciamethods/b5c619fa-def3-11e6-bf01-fe55135034f3.xml"}, "other": {"anies": [{"name": "referenceToUnitGroupDataSet", "value": {"shortDescription": [{"value": "kg N-Äq.", "lang": "de"}], "type": "unit group data set", "refObjectId": "d05bb823-ecdf-4686-8c40-bf1d9257859f", "uri": "../unitgroups/d05bb823-ecdf-4686-8c40-bf1d9257859f.xml"}}, {"value": "0.12427836965334", "module": "A1-A3"}, {"value": "0", "module": "C1"}, {"value": "0.000309473493117152", "module": "C2"}, {"value": "0", "module": "C3"}, {"value": "0.0109053093148046", "module": "C4", "scenario": "S1"}, {"value": "0.00298165920812857", "module": "C4", "scenario": "S2"}, {"value": "0", "module": "D"}]}}, {"referenceToLCIAMethodDataSet": {"shortDescription": [{"value": "Eutrophierungspotenzial Land (EP-terrestrial)", "lang": "de"}, {"value": "Eutrophication potential terrestrial (EP-terrestrial)", "lang": "en"}], "type": "LCIA method data set", "refObjectId": "b5c614d2-def3-11e6-bf01-fe55135034f3", "uri": "../lciamethods/b5c614d2-def3-11e6-bf01-fe55135034f3.xml"}, "other": {"anies": [{"name": "referenceToUnitGroupDataSet", "value": {"shortDescription": [{"value": "mol N-Äq.", "lang": "de"}], "type": "unit group data set", "refObjectId": "71b4d617-0ec9-4d3f-b65e-e438940c2401", "uri": "../unitgroups/71b4d617-0ec9-4d3f-b65e-e438940c2401.xml"}}, {"value": "3.1607650242916", "module": "A1-A3"}, {"value": "0", "module": "C1"}, {"value": "0.00354878917305199", "module": "C2"}, {"value": "0", "module": "C3"}, {"value": "0.118531536397363", "module": "C4", "scenario": "S1"}, {"value": "0.0328056961795325", "module": "C4", "scenario": "S2"}, {"value": "0", "module": "D"}]}}, {"referenceToLCIAMethodDataSet": {"shortDescription": [{"value": "Bildungspotential für troposphärisches Ozon (POCP)", "lang": "de"}, {"value": "Formation potential of tropospheric ozone photochemical oxidants (POCP)", "lang": "en"}], "type": "LCIA method data set", "refObjectId": "b5c610fe-def3-11e6-bf01-fe55135034f3", "uri": "../lciamethods/b5c610fe-def3-11e6-bf01-fe55135034f3.xml"}, "other": {"anies": [{"name": "referenceToUnitGroupDataSet", "value": {"shortDescription": [{"value": "kg NMVOC-Äq.", "lang": "de"}], "type": "unit group data set", "refObjectId": "d27c25f8-fbc1-44c6-b47b-4adbae4199c6", "uri": "../unitgroups/d27c25f8-fbc1-44c6-b47b-4adbae4199c6.xml"}}, {"value": "0.389416035121677", "module": "A1-A3"}, {"value": "0", "module": "C1"}, {"value": "0.000702897511220812", "module": "C2"}, {"value": "0", "module": "C3"}, {"value": "0.0291939347245039", "module": "C4", "scenario": "S1"}, {"value": "0.00899740746623252", "module": "C4", "scenario": "S2"}, {"value": "0", "module": "D"}]}}, {"referenceToLCIAMethodDataSet": {"shortDescription": [{"value": "Potenzial für den abiotischen Abbau nicht fossiler Ressourcen (ADPE)", "lang": "de"}, {"value": "Abiotic depletion potential for non fossil resources (ADPE)", "lang": "en"}], "type": "LCIA method data set", "refObjectId": "b2ad6494-c78d-11e6-9d9d-cec0c932ce01", "uri": "../lciamethods/b2ad6494-c78d-11e6-9d9d-cec0c932ce01.xml"}, "other": {"anies": [{"name": "referenceToUnitGroupDataSet", "value": {"shortDescription": [{"value": "kg Sb-Äq.", "lang": "de"}], "type": "unit group data set", "refObjectId": "54ccd2d9-a32a-4fc2-923d-f2c8c93e89d4", "uri": "../unitgroups/54ccd2d9-a32a-4fc2-923d-f2c8c93e89d4.xml"}}, {"value": "7.67407552393023E-06", "module": "A1-A3"}, {"value": "0", "module": "C1"}, {"value": "3.10121269793874E-08", "module": "C2"}, {"value": "0", "module": "C3"}, {"value": "9.02224850517179E-07", "module": "C4", "scenario": "S1"}, {"value": "7.52139424991425E-08", "module": "C4", "scenario": "S2"}, {"value": "0", "module": "D"}]}}, {"referenceToLCIAMethodDataSet": {"shortDescription": [{"value": "Potenzial für den abiotischen Abbau fossiler Brennstoffe (ADPF)", "lang": "de"}, {"value": "Abiotic depletion potential for fossil resources (ADPF)", "lang": "en"}], "type": "LCIA method data set", "refObjectId": "b2ad6110-c78d-11e6-9d9d-cec0c932ce01", "uri": "../lciamethods/b2ad6110-c78d-11e6-9d9d-cec0c932ce01.xml"}, "other": {"anies": [{"name": "referenceToUnitGroupDataSet", "value": {"shortDescription": [{"value": "MJ", "lang": "de"}], "type": "unit group data set", "refObjectId": "93a60a57-a3c8-11da-a746-0800200c9a66", "uri": "../unitgroups/93a60a57-a3c8-11da-a746-0800200c9a66.xml"}}, {"value": "1943.32661332607", "module": "A1-A3"}, {"value": "0", "module": "C1"}, {"value": "6.37192818406808", "module": "C2"}, {"value": "0", "module": "C3"}, {"value": "163.336059242517", "module": "C4", "scenario": "S1"}, {"value": "21.6579532815965", "module": "C4", "scenario": "S2"}, {"value": "0", "module": "D"}]}}, {"referenceToLCIAMethodDataSet": {"shortDescription": [{"value": "Wassernutzung (WDP)", "lang": "de"}, {"value": "Water use (WDP)", "lang": "en"}], "type": "LCIA method data set", "refObjectId": "b2ad66ce-c78d-11e6-9d9d-cec0c932ce01", "uri": "../lciamethods/b2ad66ce-c78d-11e6-9d9d-cec0c932ce01.xml"}, "other": {"anies": [{"name": "referenceToUnitGroupDataSet", "value": {"shortDescription": [{"value": "m^(3) Welt-Äq. entzogen", "lang": "de"}], "type": "unit group data set", "refObjectId": "6ae2df01-888e-46c8-b17d-49fa3869b476", "uri": "../unitgroups/6ae2df01-888e-46c8-b17d-49fa3869b476.xml"}}, {"value": "10.7440587536939", "module": "A1-A3"}, {"value": "0", "module": "C1"}, {"value": "0.0056521833494948", "module": "C2"}, {"value": "0", "module": "C3"}, {"value": "14.7591687992802", "module": "C4", "scenario": "S1"}, {"value": "0.178632427968837", "module": "C4", "scenario": "S2"}, {"value": "0", "module": "D"}]}}, {"referenceToLCIAMethodDataSet": {"shortDescription": [{"value": "Auftreten von Krankheiten aufgrund von Feinstaubemissionen (PM)", "lang": "de"}, {"value": "Incidence of disease due to PM emissions (PM)", "lang": "en"}], "type": "LCIA method data set", "refObjectId": "b5c602c6-def3-11e6-bf01-fe55135034f3", "uri": "../lciamethods/b5c602c6-def3-11e6-bf01-fe55135034f3.xml"}, "other": {"anies": [{"name": "referenceToUnitGroupDataSet", "value": {"shortDescription": [{"value": "Krankheitsfälle", "lang": "de"}], "type": "unit group data set", "refObjectId": "3883559b-648f-4afc-8ba2-0bd24f3affa3", "uri": "../unitgroups/3883559b-648f-4afc-8ba2-0bd24f3affa3.xml"}}, {"value": "8.39925736047916E-06", "module": "A1-A3"}, {"value": "0", "module": "C1"}, {"value": "5.24306972313746E-09", "module": "C2"}, {"value": "0", "module": "C3"}, {"value": "7.58500540383839E-07", "module": "C4", "scenario": "S1"}, {"value": "1.41929439054871E-07", "module": "C4", "scenario": "S2"}, {"value": "0", "module": "D"}]}}, {"referenceToLCIAMethodDataSet": {"shortDescription": [{"value": "Wirkung durch Exposition des Menschen mit U235 (IR)", "lang": "de"}, {"value": "Human exposure efficiency relative to U235 (IR)", "lang": "en"}], "type": "LCIA method data set", "refObjectId": "b5c632be-def3-11e6-bf01-fe55135034f3", "uri": "../lciamethods/b5c632be-def3-11e6-bf01-fe55135034f3.xml"}, "other": {"anies": [{"name": "referenceToUnitGroupDataSet", "value": {"shortDescription": [{"value": "kBq U235-Äq.", "lang": "de"}], "type": "unit group data set", "refObjectId": "456b05bf-1415-44a9-9993-02452f554c09", "uri": "../unitgroups/456b05bf-1415-44a9-9993-02452f554c09.xml"}}, {"value": "12.4192915510625", "module": "A1-A3"}, {"value": "0", "module": "C1"}, {"value": "0.00178500822347574", "module": "C2"}, {"value": "0", "module": "C3"}, {"value": "1.74558165017427", "module": "C4", "scenario": "S1"}, {"value": "0.0285623599078088", "module": "C4", "scenario": "S2"}, {"value": "0", "module": "D"}]}}, {"referenceToLCIAMethodDataSet": {"shortDescription": [{"value": "Toxizitätsvergleichseinheit für Ökosysteme (ETP-fw)", "lang": "de"}, {"value": "Comparative toxic unit for ecosystems (ETP-fw)", "lang": "en"}], "type": "LCIA method data set", "refObjectId": "ee1082d1-b0f7-43ca-a1f0-21e2a4a74511", "uri": "../lciamethods/ee1082d1-b0f7-43ca-a1f0-21e2a4a74511.xml"}, "other": {"anies": [{"name": "referenceToUnitGroupDataSet", "value": {"shortDescription": [{"value": "CTUe", "lang": "de"}], "type": "unit group data set", "refObjectId": "aa959ded-f1eb-4efb-9c5c-2d60be36b3e6", "uri": "../unitgroups/aa959ded-f1eb-4efb-9c5c-2d60be36b3e6.xml"}}, {"value": "786.403021285868", "module": "A1-A3"}, {"value": "0", "module": "C1"}, {"value": "4.56394946525985", "module": "C2"}, {"value": "0", "module": "C3"}, {"value": "75.5908725395617", "module": "C4", "scenario": "S1"}, {"value": "11.7196948323434", "module": "C4", "scenario": "S2"}, {"value": "0", "module": "D"}]}}, {"referenceToLCIAMethodDataSet": {"shortDescription": [{"value": "Toxizitätsvergleichseinheit für Menschen (krebserregend) (HTP-c)", "lang": "de"}, {"value": "Comparative toxic unit for humans (carcinogenic) (HTP-c)", "lang": "en"}], "type": "LCIA method data set", "refObjectId": "2299222a-bbd8-474f-9d4f-4dd1f18aea7c", "uri": "../lciamethods/2299222a-bbd8-474f-9d4f-4dd1f18aea7c.xml"}, "other": {"anies": [{"name": "referenceToUnitGroupDataSet", "value": {"shortDescription": [{"value": "CTUh", "lang": "de"}], "type": "unit group data set", "refObjectId": "d4c9523e-2d7e-49fd-8469-998f547d3a70", "uri": "../unitgroups/d4c9523e-2d7e-49fd-8469-998f547d3a70.xml"}}, {"value": "1.96051933359507E-07", "module": "A1-A3"}, {"value": "0", "module": "C1"}, {"value": "9.26518575322648E-11", "module": "C2"}, {"value": "0", "module": "C3"}, {"value": "2.70665462458032E-09", "module": "C4", "scenario": "S1"}, {"value": "1.81958794448645E-09", "module": "C4", "scenario": "S2"}, {"value": "0", "module": "D"}]}}, {"referenceToLCIAMethodDataSet": {"shortDescription": [{"value": "Toxizitätsvergleichseinheit für Menschen (nicht krebserregend) (HTP-nc)", "lang": "de"}, {"value": "Comparative toxic unit for humans (noncarcinogenic) (HTP-nc)", "lang": "en"}], "type": "LCIA method data set", "refObjectId": "3af763a5-b7a1-48c9-9cee-1f223481fcef", "uri": "../lciamethods/3af763a5-b7a1-48c9-9cee-1f223481fcef.xml"}, "other": {"anies": [{"name": "referenceToUnitGroupDataSet", "value": {"shortDescription": [{"value": "CTUh", "lang": "de"}], "type": "unit group data set", "refObjectId": "d4c9523e-2d7e-49fd-8469-998f547d3a70", "uri": "../unitgroups/d4c9523e-2d7e-49fd-8469-998f547d3a70.xml"}}, {"value": "3.3042552635745E-06", "module": "A1-A3"}, {"value": "0", "module": "C1"}, {"value": "4.12106289620614E-09", "module": "C2"}, {"value": "0", "module": "C3"}, {"value": "7.28959668054376E-08", "module": "C4", "scenario": "S1"}, {"value": "1.92122472911135E-07", "module": "C4", "scenario": "S2"}, {"value": "0", "module": "D"}]}}, {"referenceToLCIAMethodDataSet": {"shortDescription": [{"value": "Bodenqualitätsindex (SQP)", "lang": "de"}, {"value": "Soil quality index (SQP)", "lang": "en"}], "type": "LCIA method data set", "refObjectId": "b2ad6890-c78d-11e6-9d9d-cec0c932ce01", "uri": "../lciamethods/b2ad6890-c78d-11e6-9d9d-cec0c932ce01.xml"}, "other": {"anies": [{"name": "referenceToUnitGroupDataSet", "value": {"shortDescription": [{"value": "SQP", "lang": "de"}], "type": "unit group data set", "refObjectId": "f130951c-e67f-4f7f-8dd4-665de3974e18", "uri": "../unitgroups/f130951c-e67f-4f7f-8dd4-665de3974e18.xml"}}, {"value": "6494.18733118914", "module": "A1-A3"}, {"value": "0", "module": "C1"}, {"value": "2.66244813590662", "module": "C2"}, {"value": "0", "module": "C3"}, {"value": "51.2758344052607", "module": "C4", "scenario": "S1"}, {"value": "5.26177864862485", "module": "C4", "scenario": "S2"}, {"value": "0", "module": "D"}]}}]}, "otherAttributes": {"{http://www.indata.network/EPD/2019}epd-version": "1.2"}, "version": "1.1", "locations": "../ILCDLocations.xml"}