{"processInformation": {"dataSetInformation": {"UUID": "cf67dfdd-7a1f-4dfa-aaf7-a91f76774157", "name": {"baseName": [{"value": "EGOSILICON 300 [FARBIG] ▪ EGOSILICON 310 ▪ EGOSILICON 351 [MATT] ▪ EGOSILICON 360 [MATT] ▪ EGOSILICON 365 [MATT] ▪ EGO SPIEGELKLEBER/ LACKGLASKLEBER ▪ EGOSILICON 400", "lang": "en"}, {"value": "EGOSILICON 300 [FARBIG] ▪ EGOSILICON 310 ▪ EGOSILICON 351 [MATT] ▪ EGOSILICON 360 [MATT] ▪ EGOSILICON 365 [MATT] ▪ EGO SPIEGELKLEBER/ LACKGLASKLEBER ▪ EGOSILICON 400", "lang": "de"}], "functionalUnitFlowProperties": [{"lang": "en"}]}, "classificationInformation": {"classification": [{"class": [{"value": "Kunststoffe", "level": 0, "classId": "6"}, {"value": "Dichtmassen", "level": 1, "classId": "6.7"}, {"value": "Silikon", "level": 2, "classId": "6.7.02"}], "name": "OEKOBAU.DAT"}, {"class": [{"value": "02 Building products", "level": 0}, {"value": "Membranes, including Liquid applied and kits", "level": 1}, {"value": "Building sealants", "level": 2}], "name": "IBUCategories"}]}, "generalComment": [{"value": "Neutral curing EGOSILICONEs (EGOSILICON 300 (colored), EGOSILICON 310, EGOSILICON 351 (MATT), EGOSILICON 360 (MATT), EGOSILICON 365 (MATT), EGO SPIEGELKLEBER, EGOSILICON 400) are manufactured from reactive siloxane, colour pigments, crosslinkers, bonding agents, catalysts and optionally by using fillers and socalled\nsilicone oil. The products are formulated as moisturereactive onecomponent systems. They permanently and elastically seal joints planned for the building.\nEGOSILICONEs fulfil key functions. Ingress of moisture into the structure via the joints is prevented by EGOSILICONs. With the use of EGOSILICONEs, the fitness for use of the building and the service life are decisively extended. The product displaying the highest environmental impacts was used as a representative product for calculating the Life Cycle Assessment results (worstcase approach). For the placing on the market in the European Union/European Free Trade Association (EU/EFTA) (with the exception of Switzerland) products falling under the Regulation (EU) No 305/2011 (CPR) need a Declaration of Performance taking into consideration\neither the relevant harmonised European standard or the European Technical Assessment and the CE marking. For the application and use of the products the respective national provisions apply. Neutral curing EGOSILICONEs (EGOSILICON 300 (colored), EGOSILICON 310, EGOSILICON 351 (MATT), EGOSILICON 360 (MATT), EGOSILICON 365 (MATT), EGO SPIEGELKLEBER, EGOSILICON 400) fulfill the requirements of the application modules listed below and have the corresponding declaration of performance.", "lang": "en"}, {"value": "Neutral härtende EGOSILICONE (EGOSILICON 300 (farbig), EGOSILICON 310, EGOSILICON 351 (MATT), EGOSILICON 360 (MATT), EGOSILICON 365 (MATT), EGO SPIEGELKLEBER, EGOSILICON 400) werden aus reaktivem Siloxan, Farbpigmenten, Vernetzern, Haftvermittlern, Katalysatoren und gegebenenfalls unter Verwendung von Füllstoffen und sogenanntem Silikonöl hergestellt. Die Produkte sind als feuchtigkeitsreaktive Einkomponentensysteme formuliert. Sie dichten die für das Gebäude geplanten Fugen dauerhaft und elastisch ab. EGOSILICONEs erfüllen wichtige Funktionen. Das Eindringen von Feuchtigkeit in das Bauwerk über die Fugen wird durch EGOSILICONe verhindert. Mit dem Einsatz von EGOSILICONEs werden die Gebrauchstauglichkeit des Gebäudes und die Lebensdauer entscheidend verlängert. Das Produkt mit den höchsten Umweltauswirkungen wurde als repräsentatives Produkt für die Berechnung der Ökobilanzergebnisse (Worst-Case-Ansatz) verwendet. Für das Inverkehrbringen in der Europäischen Union/Europäischen Freihandelszone (EU/EFTA) (mit Ausnahme der Schweiz) benötigen Produkte, die unter die Verordnung (EU) Nr. 305/2011 (CPR) fallen, eine Leistungserklärung, die entweder die einschlägige harmonisierte europäische Norm oder die Europäische Technische Bewertung und die CE-Kennzeichnung berücksichtigt. Für die Anwendung und Verwendung der Produkte gelten die jeweiligen nationalen Bestimmungen. Neutral härtende EGOSILICONE (EGOSILICON 300 (farbig), EGOSILICON 310, EGOSILICON 351 (MATT), EGOSILICON 360 (MATT), EGOSILICON 365 (MATT), EGO SPIEGELKLEBER, EGOSILICON 400) erfüllen die Anforderungen der unten aufgeführten Anwendungsmodule und verfügen über die entsprechende Leistungserklärung.", "lang": "de"}]}, "quantitativeReference": {"referenceToReferenceFlow": [0]}, "time": {"referenceYear": 2025, "dataSetValidUntil": 2027, "other": {"anies": [{"name": "publicationDateOfEPD", "value": 1742774400000}]}}, "geography": {"locationOfOperationSupplyOrProduction": {"location": "RER"}}, "technology": {"technologyDescriptionAndIncludedProcesses": [{"value": "Neutral-curing EGOSILICONE (EGOSILICON 300 (colored), EGOSILICON 310, EGOSILICON 351 (MATT), EGOSILICON 360 (MATT), EGOSILICON 365 (MATT), EGO SPIEGELKLEBER, EGOSILICON 400) are manufactured from reactive siloxane, color pigments, crosslinkers, adhesion promoters, catalysts and, if necessary, fillers and so-called silicone oil. The products are formulated as moisture-reactive single-component systems. They seal the joints planned for the building permanently and elastically. EGOSILICONEs fulfill important functions. EGOSILICONEs prevent moisture from penetrating the building via the joints. The use of EGOSILICONEs significantly extends the serviceability of the building and its service life. The product with the highest environmental impact was used as the representative product for calculating the LCA results (worst-case approach). For placing on the market in the European Union/European Free Trade Association (EU/EFTA) (with the exception of Switzerland), products covered by Regulation (EU) No 305/2011 (CPR) require a Declaration of Performance that takes into account either the relevant harmonized European standard or the European Technical Assessment and CE marking. The respective national regulations apply to the application and use of the products. Neutral curing EGOSILICONE (EGOSILICON 300 (colored), EGOSILICON 310, EGOSILICON 351 (MATT), EGOSILICON 360 (MATT), EGOSILICON 365 (MATT), EGO SPIEGELKLEBER, EGOSILICON 400) meet the requirements of the application modules listed below and have the corresponding Declaration of Performance. \nTechnical data: \nThe density of the products is between 1,00 and 1,50 g/cm, other relevant technical data can be found in the manufacturers technical documentation.\n\nModule 1: Faade sealants\nThe minimum requirements on water and airtightness as per Table ZA.1 of EN 15651-1 apply: see table\n\nModule 2: Sealants for glazing \nThe minimum requirements on water and airtightness as per Table ZA.1 of EN 15651- 2 apply: see table \n\nModule 3: Sanitary sealants \nThe minimum requirements on water and airtightness as per Table ZA.1 of EN 15651-3 apply: see table\n\nModule 4: Sealants for pedestrian walkways\nThe minimum requirements on water and airtightness as per Table ZA.1 of EN 15651-4 apply: see table \nDeclared unit: \nThis EPD refers to the declared unit of 1 kg of silicone-based product, group 1; applied into the building with a density of 1.0 - 1.5 g/cm in accordance with the IBU PCR part B for construction sealants.\n\nThe results of the Life Cycle Assessment provided in this declaration have been selected from the product with the highest environmental impact (worst-case scenario).\n\nDepending on the application, a corresponding conversion factor such as the density to convert volumetric use to mass must be taken into consideration.\n\nThe Declaration type is according to EN 15804: Cradle to gate with options, modules C1–C3, and module D (A1–A3, C, D) and additional modules (A4-A5).", "lang": "en"}, {"value": "Neutral härtende EGOSILICONE (EGOSILICON 300 (farbig), EGOSILICON 310, EGOSILICON 351 (MATT), EGOSILICON 360 (MATT), EGOSILICON 365 (MATT), EGO SPIEGELKLEBER, EGOSILICON 400) werden aus reaktivem Siloxan, Farbpigmenten, Vernetzern, Haftvermittlern, Katalysatoren und gegebenenfalls unter Verwendung von Füllstoffen und sogenanntem Silikonöl hergestellt. Die Produkte sind als feuchtigkeitsreaktive Einkomponentensysteme formuliert. Sie dichten die für das Gebäude geplanten Fugen dauerhaft und elastisch ab. EGOSILICONEs erfüllen wichtige Funktionen. Das Eindringen von Feuchtigkeit in das Bauwerk über die Fugen wird durch EGOSILICONe verhindert. Mit dem Einsatz von EGOSILICONEs werden die Gebrauchstauglichkeit des Gebäudes und die Lebensdauer entscheidend verlängert. Das Produkt mit den höchsten Umweltauswirkungen wurde als repräsentatives Produkt für die Berechnung der Ökobilanzergebnisse (Worst-Case-Ansatz) verwendet. Für das Inverkehrbringen in der Europäischen Union/Europäischen Freihandelszone (EU/EFTA) (mit Ausnahme der Schweiz) benötigen Produkte, die unter die Verordnung (EU) Nr. 305/2011 (CPR) fallen, eine Leistungserklärung, die entweder die einschlägige harmonisierte europäische Norm oder die Europäische Technische Bewertung und die CE-Kennzeichnung berücksichtigt. Für die Anwendung und Verwendung der Produkte gelten die jeweiligen nationalen Bestimmungen. Neutral härtende EGOSILICONE (EGOSILICON 300 (farbig), EGOSILICON 310, EGOSILICON 351 (MATT), EGOSILICON 360 (MATT), EGOSILICON 365 (MATT), EGO SPIEGELKLEBER, EGOSILICON 400) erfüllen die Anforderungen der unten aufgeführten Anwendungsmodule und verfügen über die entsprechende Leistungserklärung. \nTechnische Daten: \nDie Dichte der Produkte liegt zwischen 1,00 und 1,50 g/cm³, weitere relevante technische Daten finden Sie in der technischen Dokumentation des Herstellers. Modul 1: Fassadendichtstoffe Es gelten die Mindestanforderungen an die Wasser- und Luftdichtheit gemäß Tabelle ZA.1 der EN 15651-1: siehe Tabelle Modul 2: Dichtstoffe für Verglasungen Es gelten die Mindestanforderungen an die Wasser- und Luftdichtheit gemäß Tabelle ZA.1 der EN 15651- 2 gelten: siehe Tabelle Modul 3: Sanitärdichtstoffe Es gelten die Mindestanforderungen an die Wasser- und Luftdichtheit gemäß Tabelle ZA.1 der EN 15651-3: siehe Tabelle Modul 4: Dichtstoffe für Fußgängerüberwege Es gelten die Mindestanforderungen an die Wasser- und Luftdichtheit gemäß Tabelle ZA.1 der EN 15651-4: siehe Tabelle \nDeklarierte Einheit: \nDiese EPD bezieht sich auf die deklarierte Einheit von 1 kg silikonbasiertem Produkt, Gruppe 1, das mit einer Dichte von 1,0 - 1,5 g/cm³ gemäß IBU PCR Teil B für Bauwerksabdichtungen in das Gebäude eingebracht wird. Die in dieser Deklaration angegebenen Ergebnisse der Ökobilanz wurden aus dem Produkt mit den höchsten Umweltauswirkungen (Worst-Case-Szenario) ausgewählt. Je nach Anwendung muss ein entsprechender Umrechnungsfaktor wie die Dichte zur Umrechnung des volumetrischen Verbrauchs in Masse berücksichtigt werden. Der Deklarationstyp entspricht der EN 15804: Cradle to Gate mit Optionen, Modulen C1-C3 und Modul D (A1-A3, C, D) und Zusatzmodulen (A4-A5).", "lang": "de"}], "technologicalApplicability": [{"value": "Module 1: Faade sealants\nSilicone-based products are used for the elastic sealing of joints. The areas of application for faade sealants include expansion joints (movement joints) and/or connection joints already existing in exterior walls and on window and door frames (including the inside section). All these sealants fulfil key functions of the building.\n\nModule 2: Sealants for glazing \nSilicone-based products are used for the elastic sealing of joints which may be subject to movement. Sealants for glazing are used in the following areas: (i)Glass to glass (ii)Glass to frame (iii)Glass to porous substrates \n\nModule 3: Sanitary sealants \nThe areas of application for silicone-based sanitary sealants are joints in sanitary areas and kitchens. Joints sealed using sanitary sealants comprise connection joints between sanitary furnishings and the wall, connection joints between the floor and wall or movement joints across surfaces, for example.\n\nModule 4: Sealants for pedestrian walkways\nThe areas of application for silicone-based sealants for pedestrian walkways are floor joints designed for pedestrian walkways, public areas, movement joints between concrete slabs, areas with pedestrian load, areas used with trolleys, walkable floors, balconies, terraces, warehouses.", "lang": "en"}, {"value": "Modul 1: Fassadendichtstoffe \nProdukte auf Silikonbasis werden zur elastischen Abdichtung von Fugen eingesetzt. Zu den Anwendungsbereichen von Fassadendichtstoffen gehören Dehnungsfugen (Bewegungsfugen) und/oder bereits vorhandene Anschlussfugen in Außenwänden sowie an Fenster- und Türrahmen (auch im Innenbereich). Alle diese Dichtstoffe erfüllen wichtige Funktionen des Gebäudes.\n\n \n\nModul 2: Dichtstoffe für Verglasungen \n\nProdukte auf Silikonbasis werden für die elastische Abdichtung von Fugen verwendet, die Bewegungen ausgesetzt sein können. Dichtstoffe für Verglasungen werden in folgenden Bereichen eingesetzt: (i) Glas zu Glas (ii) Glas zu Rahmen (iii) Glas zu porösen Untergründen \n\n \n\nModul 3: Sanitärdichtstoffe \n\nDie Anwendungsbereiche für Sanitärdichtstoffe auf Silikonbasis sind Fugen im Sanitärbereich und in Küchen. Fugen, die mit Sanitärdichtstoffen abgedichtet werden, sind z.B. Anschlussfugen zwischen Sanitäreinrichtung und Wand, Anschlussfugen zwischen Boden und Wand oder Bewegungsfugen über Flächen.\n\n \n\nModul 4: Dichtstoffe für Fußgängerwege\n\nAnwendungsbereiche für Silikondichtstoffe für Fußgängerwege sind Bodenfugen für Fußgängerwege, öffentliche Bereiche, Bewegungsfugen zwischen Betonplatten, Bereiche mit Fußgängerbelastung, Bereiche mit Laufkatzen, begehbare Böden, Balkone, Terrassen, Lagerhallen.", "lang": "de"}]}}, "modellingAndValidation": {"LCIMethodAndAllocation": {"typeOfDataSet": "EPD", "referenceToLCAMethodDetails": [{"shortDescription": [{"value": "Building sealants.pdf", "lang": "en"}], "type": "source data set", "refObjectId": "c7d774e2-ffc2-4cc0-9ba3-dc6558dc8947"}], "other": {"anies": [{"name": "subType", "value": "template dataset"}]}}, "dataSourcesTreatmentAndRepresentativeness": {"referenceToDataSource": [{"shortDescription": [{"value": "GaBi Database (all versions)", "lang": "en"}], "type": "source data set", "refObjectId": "28d74cc0-db8b-4d7e-bc44-5f6d56ce0c4a"}, {"shortDescription": [{"value": "GaBi database SP40 2020", "lang": "en"}], "type": "source data set", "refObjectId": "0115289e-52f0-4920-bc7e-57b1c96aec8d"}], "useAdviceForDataSet": [{"value": "Scope: \nThis is a manufacturer-individualised EPD based on model declaration 'Silicone-based products, group 1' (EPD-DBC-20220179-IBF1-EN) from Deutsche Bauchemie e.V. (DBC), European Federation for Construction Chemicals (EFCC), Association of the European Adhesive and Sealant Industry (FEICA) and Industrieverband Klebstoffe e.V. (IVK) in which the product exhibiting the highest environmental impact in a particular group was selected from the group to calculate the LCA. This verified EPD entitles the holder to bear the symbol of the Institut Bauen und Umwelt e.V.. It exclusively applies to products produced in Europe and applies to a period of five years from the date of issue. This EPD may be used by members of DBC, EFCC, FEICA and IVK and their members provided. It\nhas been proven that the respective product can be represented by this EPD. \nSystem boundary: \nModules A1, A2 and A3 are taken into consideration in the LCA:\n\n- A1 Production of preliminary products\n\n- A2 Transport to the plant\n\n- A3 Production incl. provision of energy, production of packaging as well as auxiliaries and consumables and waste treatment\n\n- A4 Transport to site\n\n- A5 Installation, product applied into the building during A5 phase operations and packaging disposal. This stage considers VOC emissions during the installation phase. The declared product does not contain substances in(to) the formulation that directly emit as VOC, but VOCs are generated by a chemical reaction that is occurring during this phase.\n\nThe end of life for the packaging material considered is described below:\n\n-Incineration, for materials like plastic, paper and wood.\n\n-C1-C2-C3-D\n\nThe building deconstruction (demolition process) takes place in the C1 module which considers energy generation and consumption of diesel and all the emissions connected with the fuel-burning process to run the machines. After the demolition, the product is transported to the end-of-life processing (C2 module) where all the impacts related to the transport processes are considered. For precautionary principle and as a worst-case scenario, thermal treatment is the only end-of-life scenario considered. This is modelled by the incineration process (module C3) where the product ends its life cycle.\n\nModule D accounts for potential benefits that are beyond the defined system boundaries. Credits are generated during the incineration of wastes and related electricity produced that are occurring in the A5 module.", "lang": "en"}, {"value": "Gültigkeitsbereich: \nDies ist eine herstellerindividuelle EPD basierend auf der Modelldeklaration \"Silikonhaltige Produkte, Gruppe 1\" (EPD-DBC-20220179-IBF1-EN) der Deutschen Bauchemie e.V. (DBC), Europäischer Verband für Bauchemie Bauchemie (EFCC), dem Verband der Europäischen Klebstoff- und Dichtstoffindustrie\nKlebstoffindustrie (FEICA) und des Industrieverbands Klebstoffe e.V. (IVK), in dem das\nProdukt mit den höchsten Umweltauswirkungen in einer bestimmten Gruppe aus der Gruppe ausgewählt wurde, um die Ökobilanz zu berechnen.  \nSystemgrenze: \nDie Module A1, A2 und A3 werden in der Ökobilanz berücksichtigt: - A1 Produktion von Vorprodukten - A2 Transport zum Werk - A3 Produktion inkl. Energiebereitstellung, Herstellung von Verpackungen sowie Hilfs- und Betriebsstoffen und Abfallbehandlung - A4 Transport zur Baustelle - A5 Installation, Produktanwendung im Gebäude während der Phase A5 und Entsorgung der Verpackung. Diese Phase berücksichtigt die VOC-Emissionen während der Installationsphase. Das deklarierte Produkt enthält keine Stoffe in der Formulierung, die direkt als VOC emittieren, aber VOCs werden durch eine chemische Reaktion erzeugt, die in dieser Phase stattfindet. Das Ende der Lebensdauer des betrachteten Verpackungsmaterials wird im Folgenden beschrieben: - Verbrennung, für Materialien wie Kunststoff, Papier und Holz. -C1-C2-C3-D Der Rückbau des Gebäudes (Abriss) findet im Modul C1 statt, das die Energieerzeugung und den Verbrauch von Diesel und alle mit der Verbrennung des Kraftstoffs zum Betrieb der Maschinen verbundenen Emissionen berücksichtigt. Nach dem Abriss wird das Produkt zur End-of-Life-Verarbeitung (Modul C2) transportiert, wo alle mit den Transportprozessen verbundenen Auswirkungen berücksichtigt werden. Aus Gründen des Vorsorgeprinzips und als Worst-Case-Szenario wird als einziges End-of-Life-Szenario die thermische Behandlung berücksichtigt. Dies wird durch den Verbrennungsprozess (Modul C3) modelliert, bei dem das Produkt seinen Lebenszyklus beendet. Modul D berücksichtigt mögliche Vorteile, die über die definierten Systemgrenzen hinausgehen. Gutschriften werden bei der Verbrennung von Abfällen und der damit verbundenen Stromerzeugung generiert, die im Modul A5 vorkommen.", "lang": "de"}], "other": {"anies": [{"name": "referenceToOriginalEPD", "value": {"shortDescription": {"value": "EGOSILICON 300 [FARBIG] ▪ EGOSILICON 310 ▪ EGOSILICON 351 [MATT] ▪ EGOSILICON 360 [MATT] ▪ EGOSILICON 365 [MATT] ▪ EGO SPIEGELKLEBER/ LACKGLASKLEBER ▪ EGOSILICON 400.pdf", "defaultValue": "EGOSILICON 300 [FARBIG] ▪ EGOSILICON 310 ▪ EGOSILICON 351 [MATT] ▪ EGOSILICON 360 [MATT] ▪ EGOSILICON 365 [MATT] ▪ EGO SPIEGELKLEBER/ LACKGLASKLEBER ▪ EGOSILICON 400.pdf", "lstrings": [{"lang": "en", "value": "EGOSILICON 300 [FARBIG] ▪ EGOSILICON 310 ▪ EGOSILICON 351 [MATT] ▪ EGOSILICON 360 [MATT] ▪ EGOSILICON 365 [MATT] ▪ EGO SPIEGELKLEBER/ LACKGLASKLEBER ▪ EGOSILICON 400.pdf"}]}, "type": "source data set", "uuid": {"uuid": "768992c6-483b-4c6a-8383-3e6ea753e6ef"}, "refObjectId": "768992c6-483b-4c6a-8383-3e6ea753e6ef", "resourceURLs": ["https://oekobaudat.de/OEKOBAU.DAT/resource/sources/768992c6-483b-4c6a-8383-3e6ea753e6ef/EGOSILICON_300_FARBIG_EGOSILICON_310_EGOSILICON_351_MATT_EGOSILICON_360_MATT_EGOSILICON_365_MATT_EGO_SPIEGELKLEBER_LACKGLASKLEBER_EGOSILICON_400_23280.pdf?version=00.01.000"]}}]}}, "validation": {"review": [{"referenceToNameOfReviewerAndInstitution": [{"shortDescription": [{"value": "Institut Bauen und Umwelt e. V.", "lang": "en"}], "type": "contact data set", "refObjectId": "d111dbec-b024-4be5-86c5-752d6eb2cf95", "uri": "../contacts/d111dbec-b024-4be5-86c5-752d6eb2cf95.xml"}], "type": "Accredited third party review"}]}, "complianceDeclarations": {"compliance": [{"referenceToComplianceSystem": {"shortDescription": [{"value": "DIN EN 15804+A2", "lang": "en"}], "type": "source data set", "refObjectId": "c0016b33-8cf7-415c-ac6e-deba0d21440d", "uri": "../sources/c0016b33-8cf7-415c-ac6e-deba0d21440d.xml"}}, {"referenceToComplianceSystem": {"shortDescription": [{"value": "ISO 14025", "lang": "en"}], "type": "source data set", "refObjectId": "4f2eb655-6e44-4874-a95a-e28f5442cd4d", "uri": "../sources/4f2eb655-6e44-4874-a95a-e28f5442cd4d.xml"}}]}}, "administrativeInformation": {"commissionerAndGoal": {"referenceToCommissioner": [{"shortDescription": [{"value": "EGO Dichtstoffwerke GmbH & Co. Betriebs KG", "lang": "en"}], "type": "contact data set", "refObjectId": "9088e8a3-8716-4acb-b807-8826cacbbe60", "uri": "../contacts/9088e8a3-8716-4acb-b807-8826cacbbe60.xml"}]}, "dataGenerator": {"referenceToPersonOrEntityGeneratingTheDataSet": [{"shortDescription": [{"value": "Sphera Solutions GmbH", "lang": "en"}], "type": "contact data set", "refObjectId": "623edf96-39d1-4e6f-9892-674c7228546b", "uri": "../contacts/623edf96-39d1-4e6f-9892-674c7228546b.xml"}]}, "dataEntryBy": {"timeStamp": 1742774400000, "referenceToDataSetFormat": [{"shortDescription": [{"value": "ILCD Format", "lang": "en"}], "type": "source data set", "refObjectId": "a97a0155-0234-4b87-b4ce-a45da52f2a40", "uri": "../sources/a97a0155-0234-4b87-b4ce-a45da52f2a40.xml"}, {"shortDescription": [{"value": "EPD-Datenformaterweiterungen v1.2", "lang": "de"}, {"value": "EPD Data Format Extensions v1.2", "lang": "en"}], "type": "source data set", "refObjectId": "a29449fd-aa2f-4de8-b5d7-4b06b43c6fde", "uri": "../sources/a29449fd-aa2f-4de8-b5d7-4b06b43c6fde.xml"}]}, "publicationAndOwnership": {"dataSetVersion": "00.01.000", "referenceToPrecedingDataSetVersion": [{"shortDescription": [{"value": "Silicone-based products, group 1 ", "lang": "en"}], "type": "process data set", "refObjectId": "ebacaeb0-8fa2-48c9-bba4-bd290f1a681d", "uri": "../processes/ebacaeb0-8fa2-48c9-bba4-bd290f1a681d.xml"}], "referenceToRegistrationAuthority": {"shortDescription": [{"value": "Institut Bauen und Umwelt e. V.", "lang": "en"}], "type": "contact data set", "refObjectId": "d111dbec-b024-4be5-86c5-752d6eb2cf95", "uri": "../contacts/d111dbec-b024-4be5-86c5-752d6eb2cf95.xml"}, "registrationNumber": "EPD-DBC-EGO-20250171-IBF1-EN", "referenceToOwnershipOfDataSet": {"shortDescription": [{"value": "EGO Dichtstoffwerke GmbH & Co. Betriebs KG", "lang": "en"}], "type": "contact data set", "refObjectId": "9088e8a3-8716-4acb-b807-8826cacbbe60", "uri": "../contacts/9088e8a3-8716-4acb-b807-8826cacbbe60.xml"}, "copyright": true, "licenseType": "Free of charge for all users and uses", "accessRestrictions": [{"value": "None", "lang": "en"}], "other": {"anies": [{"name": "referenceToPublisher", "value": {"shortDescription": [{"value": "Institut Bauen und Umwelt e. V.", "lang": "en"}], "type": "contact data set", "refObjectId": "d111dbec-b024-4be5-86c5-752d6eb2cf95", "uri": "../contacts/d111dbec-b024-4be5-86c5-752d6eb2cf95.xml"}}]}}}, "exchanges": {"exchange": [{"dataSetInternalID": 0, "referenceToFlowDataSet": {"shortDescription": [{"value": "EGOSILICON 300 [FARBIG] ▪ EGOSILICON 310 ▪ EGOSILICON 351 [MATT] ▪ EGOSILICON 360 [MATT] ▪ EGOSILICON 365 [MATT] ▪ EGO SPIEGELKLEBER/ LACKGLASKLEBER ▪ EGOSILICON 400 (Silikonbasierte Produkte, Gruppe 1)", "lang": "en"}], "type": "flow data set", "refObjectId": "85bb52bb-eb47-01da-5588-acf483149b91", "uri": "../flows/85bb52bb-eb47-01da-5588-acf483149b91.xml"}, "meanAmount": 1.0, "referencesToDataSource": {}, "referenceFlow": true, "resolvedFlowVersion": "00.01.000", "resultingflowAmount": 1.0, "flowProperties": [{"name": [{"lang": "en", "value": "Mass"}, {"lang": "de", "value": "Masse"}], "uuid": "93a60a56-a3c8-11da-a746-0800200b9a66", "referenceFlowProperty": true, "meanValue": 1.0, "referenceUnit": "kg", "unitGroupUUID": "ad38d542-3fe9-439d-9b95-2f5f7752acaf"}], "materialProperties": [{"name": "gross density", "value": "1400.0", "unit": "kg/m^3", "unitDescription": "kilograms per cubic metre"}], "typeOfFlow": "Product flow", "classification": {"classHierarchy": "Kunststoffe / Dichtmassen / Silikon", "name": "OEKOBAU.DAT"}}, {"dataSetInternalID": 1, "referenceToFlowDataSet": {"shortDescription": [{"value": "Renewable primary energy as energy carrier (PERE)", "lang": "en"}, {"value": "Erneuerbare Primärenergie als Energieträger (PERE)", "lang": "de"}], "type": "flow data set", "refObjectId": "20f32be5-0398-4288-9b6d-accddd195317", "uri": "../flows/20f32be5-0398-4288-9b6d-accddd195317.xml"}, "exchange direction": "INPUT", "other": {"anies": [{"name": "referenceToUnitGroupDataSet", "value": {"shortDescription": [{"value": "MJ", "lang": "en"}], "type": "unit group data set", "refObjectId": "93a60a57-a3c8-11da-a746-0800200c9a66", "uri": "../unitgroups/93a60a57-a3c8-11da-a746-0800200c9a66.xml"}}, {"value": "37.658608844325", "module": "A1-A3"}, {"value": "0.04346010975", "module": "A4"}, {"value": "1.307968362", "module": "A5"}, {"value": "1.201458581E-05", "module": "C1"}, {"value": "0.0005245659266", "module": "C2"}, {"value": "0.09362619296", "module": "C3"}, {"value": "-2.168403909", "module": "D"}]}, "resolvedFlowVersion": "38.00.000", "flowProperties": [], "typeOfFlow": "Other flow", "classification": {"classHierarchy": "Quantities", "name": "GaBiCategories"}}, {"dataSetInternalID": 2, "referenceToFlowDataSet": {"shortDescription": [{"value": "Renewable primary energy resources as material utilization (PERM)", "lang": "en"}, {"value": "Erneuerbare Primärenergie zur stofflichen Nutzung (PERM)", "lang": "de"}], "type": "flow data set", "refObjectId": "fb3ec0de-548d-4508-aea5-00b73bf6f702", "uri": "../flows/fb3ec0de-548d-4508-aea5-00b73bf6f702.xml"}, "exchange direction": "INPUT", "other": {"anies": [{"name": "referenceToUnitGroupDataSet", "value": {"shortDescription": [{"value": "MJ", "lang": "en"}], "type": "unit group data set", "refObjectId": "93a60a57-a3c8-11da-a746-0800200c9a66", "uri": "../unitgroups/93a60a57-a3c8-11da-a746-0800200c9a66.xml"}}, {"value": "0.905", "module": "A1-A3"}, {"value": "0", "module": "A4"}, {"value": "-0.905", "module": "A5"}, {"value": "0", "module": "C1"}, {"value": "0", "module": "C2"}, {"value": "0", "module": "C3"}, {"value": "0", "module": "D"}]}, "resolvedFlowVersion": "38.00.000", "flowProperties": [], "typeOfFlow": "Other flow", "classification": {"classHierarchy": "Quantities", "name": "GaBiCategories"}}, {"dataSetInternalID": 3, "referenceToFlowDataSet": {"shortDescription": [{"value": "Total use of renewable primary energy resources (PERT)", "lang": "en"}, {"value": "Total erneuerbare Primärenergie (PERT)", "lang": "de"}], "type": "flow data set", "refObjectId": "53f97275-fa8a-4cdd-9024-65936002acd0", "uri": "../flows/53f97275-fa8a-4cdd-9024-65936002acd0.xml"}, "exchange direction": "INPUT", "other": {"anies": [{"name": "referenceToUnitGroupDataSet", "value": {"shortDescription": [{"value": "MJ", "lang": "en"}], "type": "unit group data set", "refObjectId": "93a60a57-a3c8-11da-a746-0800200c9a66", "uri": "../unitgroups/93a60a57-a3c8-11da-a746-0800200c9a66.xml"}}, {"value": "38.563608844325", "module": "A1-A3"}, {"value": "0.04346010975", "module": "A4"}, {"value": "0.4029683623", "module": "A5"}, {"value": "1.201458581E-05", "module": "C1"}, {"value": "0.0005245659266", "module": "C2"}, {"value": "0.09362619296", "module": "C3"}, {"value": "-2.168403909", "module": "D"}]}, "resolvedFlowVersion": "38.00.000", "flowProperties": [], "typeOfFlow": "Other flow", "classification": {"classHierarchy": "Quantities / Environmental quantities / EPD EN 15804 / LCI indicators", "name": "GaBiCategories"}}, {"dataSetInternalID": 4, "referenceToFlowDataSet": {"shortDescription": [{"value": "Non renewable primary energy as energy carrier (PENRE)", "lang": "en"}, {"value": "Nicht-erneuerbare Primärenergie als Energieträger (PENRE)", "lang": "de"}], "type": "flow data set", "refObjectId": "ac857178-2b45-46ec-892a-a9a4332f0372", "uri": "../flows/ac857178-2b45-46ec-892a-a9a4332f0372.xml"}, "exchange direction": "INPUT", "other": {"anies": [{"name": "referenceToUnitGroupDataSet", "value": {"shortDescription": [{"value": "MJ", "lang": "en"}], "type": "unit group data set", "refObjectId": "93a60a57-a3c8-11da-a746-0800200c9a66", "uri": "../unitgroups/93a60a57-a3c8-11da-a746-0800200c9a66.xml"}}, {"value": "81.08864107578", "module": "A1-A3"}, {"value": "0.7739228357", "module": "A4"}, {"value": "8.43164157", "module": "A5"}, {"value": "0.003814072491", "module": "C1"}, {"value": "0.1665252971", "module": "C2"}, {"value": "10.00218467", "module": "C3"}, {"value": "-10.55152613", "module": "D"}]}, "resolvedFlowVersion": "38.00.000", "flowProperties": [], "typeOfFlow": "Other flow", "classification": {"classHierarchy": "Quantities", "name": "GaBiCategories"}}, {"dataSetInternalID": 5, "referenceToFlowDataSet": {"shortDescription": [{"value": "Non renewable primary energy as material utilization (PENRM)", "lang": "en"}, {"value": "Nicht-erneuerbare Primärenergie zur stofflichen Nutzung (PENRM)", "lang": "de"}], "type": "flow data set", "refObjectId": "1421caa0-679d-4bf4-b282-0eb850ccae27", "uri": "../flows/1421caa0-679d-4bf4-b282-0eb850ccae27.xml"}, "exchange direction": "INPUT", "other": {"anies": [{"name": "referenceToUnitGroupDataSet", "value": {"shortDescription": [{"value": "MJ", "lang": "en"}], "type": "unit group data set", "refObjectId": "93a60a57-a3c8-11da-a746-0800200c9a66", "uri": "../unitgroups/93a60a57-a3c8-11da-a746-0800200c9a66.xml"}}, {"value": "16.81", "module": "A1-A3"}, {"value": "0", "module": "A4"}, {"value": "-7.36", "module": "A5"}, {"value": "0", "module": "C1"}, {"value": "0", "module": "C2"}, {"value": "-9.45", "module": "C3"}, {"value": "0", "module": "D"}]}, "resolvedFlowVersion": "38.00.000", "flowProperties": [], "typeOfFlow": "Other flow", "classification": {"classHierarchy": "Quantities", "name": "GaBiCategories"}}, {"dataSetInternalID": 6, "referenceToFlowDataSet": {"shortDescription": [{"value": "Total use of non renewable primary energy resources (PENRT)", "lang": "en"}, {"value": "Total nicht erneuerbare Primärenergie (PENRT)", "lang": "de"}], "type": "flow data set", "refObjectId": "06159210-646b-4c8d-8583-da9b3b95a6c1", "uri": "../flows/06159210-646b-4c8d-8583-da9b3b95a6c1.xml"}, "exchange direction": "INPUT", "other": {"anies": [{"name": "referenceToUnitGroupDataSet", "value": {"shortDescription": [{"value": "MJ", "lang": "en"}], "type": "unit group data set", "refObjectId": "93a60a57-a3c8-11da-a746-0800200c9a66", "uri": "../unitgroups/93a60a57-a3c8-11da-a746-0800200c9a66.xml"}}, {"value": "97.89864107978", "module": "A1-A3"}, {"value": "0.7739228357", "module": "A4"}, {"value": "1.07164157", "module": "A5"}, {"value": "0.003814072491", "module": "C1"}, {"value": "0.1665252971", "module": "C2"}, {"value": "0.5521846688", "module": "C3"}, {"value": "-10.55152613", "module": "D"}]}, "resolvedFlowVersion": "38.00.000", "flowProperties": [], "typeOfFlow": "Other flow", "classification": {"classHierarchy": "Quantities / Environmental quantities / EPD EN 15804 / LCI indicators", "name": "GaBiCategories"}}, {"dataSetInternalID": 7, "referenceToFlowDataSet": {"shortDescription": [{"value": "Use of secondary material (SM)", "lang": "en"}, {"value": "Einsatz von Sekundärstoffen (SM)", "lang": "de"}], "type": "flow data set", "refObjectId": "c6a1f35f-2d09-4f54-8dfb-97e502e1ce92", "uri": "../flows/c6a1f35f-2d09-4f54-8dfb-97e502e1ce92.xml"}, "exchange direction": "INPUT", "other": {"anies": [{"name": "referenceToUnitGroupDataSet", "value": {"shortDescription": [{"value": "kg", "lang": "en"}], "type": "unit group data set", "refObjectId": "ad38d542-3fe9-439d-9b95-2f5f7752acaf", "uri": "../unitgroups/ad38d542-3fe9-439d-9b95-2f5f7752acaf.xml"}}, {"value": "0", "module": "A1-A3"}, {"value": "0", "module": "A4"}, {"value": "0", "module": "A5"}, {"value": "0", "module": "C1"}, {"value": "0", "module": "C2"}, {"value": "0", "module": "C3"}, {"value": "0", "module": "D"}]}, "resolvedFlowVersion": "38.00.000", "flowProperties": [], "typeOfFlow": "Other flow", "classification": {"classHierarchy": "Quantities / Environmental quantities / EPD EN 15804 / LCI indicators", "name": "GaBiCategories"}}, {"dataSetInternalID": 8, "referenceToFlowDataSet": {"shortDescription": [{"value": "Use of renewable secondary fuels (RSF)", "lang": "en"}, {"value": "Erneuerbare Sekundärbrennstoffe (RSF)", "lang": "de"}], "type": "flow data set", "refObjectId": "64333088-a55f-4aa2-9a31-c10b07816787", "uri": "../flows/64333088-a55f-4aa2-9a31-c10b07816787.xml"}, "exchange direction": "INPUT", "other": {"anies": [{"name": "referenceToUnitGroupDataSet", "value": {"shortDescription": [{"value": "MJ", "lang": "en"}], "type": "unit group data set", "refObjectId": "93a60a57-a3c8-11da-a746-0800200c9a66", "uri": "../unitgroups/93a60a57-a3c8-11da-a746-0800200c9a66.xml"}}, {"value": "0", "module": "A1-A3"}, {"value": "0", "module": "A4"}, {"value": "0", "module": "A5"}, {"value": "0", "module": "C1"}, {"value": "0", "module": "C2"}, {"value": "0", "module": "C3"}, {"value": "0", "module": "D"}]}, "resolvedFlowVersion": "38.00.000", "flowProperties": [], "typeOfFlow": "Other flow", "classification": {"classHierarchy": "Quantities / Environmental quantities / EPD EN 15804 / LCI indicators", "name": "GaBiCategories"}}, {"dataSetInternalID": 9, "referenceToFlowDataSet": {"shortDescription": [{"value": "Use of non renewable secondary fuels (NRSF)", "lang": "en"}, {"value": "Nicht erneuerbare Sekundärbrennstoffe (NRSF)", "lang": "de"}], "type": "flow data set", "refObjectId": "89def144-d39a-4287-b86f-efde453ddcb2", "uri": "../flows/89def144-d39a-4287-b86f-efde453ddcb2.xml"}, "exchange direction": "INPUT", "other": {"anies": [{"name": "referenceToUnitGroupDataSet", "value": {"shortDescription": [{"value": "MJ", "lang": "en"}], "type": "unit group data set", "refObjectId": "93a60a57-a3c8-11da-a746-0800200c9a66", "uri": "../unitgroups/93a60a57-a3c8-11da-a746-0800200c9a66.xml"}}, {"value": "0", "module": "A1-A3"}, {"value": "0", "module": "A4"}, {"value": "0", "module": "A5"}, {"value": "0", "module": "C1"}, {"value": "0", "module": "C2"}, {"value": "0", "module": "C3"}, {"value": "0", "module": "D"}]}, "resolvedFlowVersion": "38.00.000", "flowProperties": [], "typeOfFlow": "Other flow", "classification": {"classHierarchy": "Quantities / Environmental quantities / EPD EN 15804 / LCI indicators", "name": "GaBiCategories"}}, {"dataSetInternalID": 10, "referenceToFlowDataSet": {"shortDescription": [{"value": "Use of net fresh water (FW)", "lang": "en"}, {"value": "Einsatz von Süßwasserressourcen (FW)", "lang": "de"}], "type": "flow data set", "refObjectId": "3cf952c8-f3a4-461d-8c96-96456ca62246", "uri": "../flows/3cf952c8-f3a4-461d-8c96-96456ca62246.xml"}, "exchange direction": "INPUT", "other": {"anies": [{"name": "referenceToUnitGroupDataSet", "value": {"shortDescription": [{"value": "m^3", "lang": "en"}], "type": "unit group data set", "refObjectId": "cd950537-0a98-4044-9ba7-9f9a68d0a504", "uri": "../unitgroups/cd950537-0a98-4044-9ba7-9f9a68d0a504.xml"}}, {"value": "0.0518259146435928", "module": "A1-A3"}, {"value": "5.032382486E-05", "module": "A4"}, {"value": "0.00192091253", "module": "A5"}, {"value": "2.155216422E-08", "module": "C1"}, {"value": "9.409838324E-07", "module": "C2"}, {"value": "0.003702831056", "module": "C3"}, {"value": "-0.002511521964", "module": "D"}]}, "resolvedFlowVersion": "38.00.000", "flowProperties": [], "typeOfFlow": "Other flow", "classification": {"classHierarchy": "Quantities / Environmental quantities / EPD EN 15804 / LCI indicators", "name": "GaBiCategories"}}, {"dataSetInternalID": 11, "referenceToFlowDataSet": {"shortDescription": [{"value": "Hazardous waste disposed (HWD)", "lang": "en"}, {"value": "Gefährlicher Abfall zur Deponie (HWD)", "lang": "de"}], "type": "flow data set", "refObjectId": "430f9e0f-59b2-46a0-8e0d-55e0e84948fc", "uri": "../flows/430f9e0f-59b2-46a0-8e0d-55e0e84948fc.xml"}, "exchange direction": "OUTPUT", "other": {"anies": [{"name": "referenceToUnitGroupDataSet", "value": {"shortDescription": [{"value": "kg", "lang": "en"}], "type": "unit group data set", "refObjectId": "ad38d542-3fe9-439d-9b95-2f5f7752acaf", "uri": "../unitgroups/ad38d542-3fe9-439d-9b95-2f5f7752acaf.xml"}}, {"value": "7.38948962425071E-07", "module": "A1-A3"}, {"value": "3.601591939E-08", "module": "A4"}, {"value": "7.471907997E-09", "module": "A5"}, {"value": "3.699446997E-13", "module": "C1"}, {"value": "1.615206611E-11", "module": "C2"}, {"value": "1.769689708E-09", "module": "C3"}, {"value": "-4.198599327E-09", "module": "D"}]}, "resolvedFlowVersion": "38.00.000", "flowProperties": [], "typeOfFlow": "Other flow", "classification": {"classHierarchy": "Quantities / Environmental quantities / EPD EN 15804 / LCI indicators", "name": "GaBiCategories"}}, {"dataSetInternalID": 12, "referenceToFlowDataSet": {"shortDescription": [{"value": "Non hazardous waste disposed (NHWD)", "lang": "en"}, {"value": "Entsorgter nicht gefährlicher Abfall (NHWD)", "lang": "de"}], "type": "flow data set", "refObjectId": "b29ef66b-e286-4afa-949f-62f1a7b4d7fa", "uri": "../flows/b29ef66b-e286-4afa-949f-62f1a7b4d7fa.xml"}, "exchange direction": "OUTPUT", "other": {"anies": [{"name": "referenceToUnitGroupDataSet", "value": {"shortDescription": [{"value": "kg", "lang": "en"}], "type": "unit group data set", "refObjectId": "ad38d542-3fe9-439d-9b95-2f5f7752acaf", "uri": "../unitgroups/ad38d542-3fe9-439d-9b95-2f5f7752acaf.xml"}}, {"value": "1.26887507485091", "module": "A1-A3"}, {"value": "0.0001184398105", "module": "A4"}, {"value": "0.01735299729", "module": "A5"}, {"value": "3.899640619E-07", "module": "C1"}, {"value": "1.702612664E-05", "module": "C2"}, {"value": "0.1364908888", "module": "C3"}, {"value": "-0.004725645142", "module": "D"}]}, "resolvedFlowVersion": "38.00.000", "flowProperties": [], "typeOfFlow": "Other flow", "classification": {"classHierarchy": "Quantities / Environmental quantities / EPD EN 15804 / LCI indicators", "name": "GaBiCategories"}}, {"dataSetInternalID": 13, "referenceToFlowDataSet": {"shortDescription": [{"value": "Radioactive waste disposed (RWD)", "lang": "en"}, {"value": "Entsorgter radioaktiver Abfall (RWD)", "lang": "de"}], "type": "flow data set", "refObjectId": "3449546e-52ad-4b39-b809-9fb77cea8ff6", "uri": "../flows/3449546e-52ad-4b39-b809-9fb77cea8ff6.xml"}, "exchange direction": "OUTPUT", "other": {"anies": [{"name": "referenceToUnitGroupDataSet", "value": {"shortDescription": [{"value": "kg", "lang": "en"}], "type": "unit group data set", "refObjectId": "ad38d542-3fe9-439d-9b95-2f5f7752acaf", "uri": "../unitgroups/ad38d542-3fe9-439d-9b95-2f5f7752acaf.xml"}}, {"value": "0.0039582605034122", "module": "A1-A3"}, {"value": "9.579122821E-07", "module": "A4"}, {"value": "4.486649749E-05", "module": "A5"}, {"value": "4.093764604E-09", "module": "C1"}, {"value": "1.787368668E-07", "module": "C2"}, {"value": "2.512269658E-05", "module": "C3"}, {"value": "-0.0007402472833", "module": "D"}]}, "resolvedFlowVersion": "38.00.000", "flowProperties": [], "typeOfFlow": "Other flow", "classification": {"classHierarchy": "Quantities / Environmental quantities / EPD EN 15804 / LCI indicators", "name": "GaBiCategories"}}, {"dataSetInternalID": 14, "referenceToFlowDataSet": {"shortDescription": [{"value": "Components for re-use (CRU)", "lang": "en"}, {"value": "Komponenten für die Wiederverwendung (CRU)", "lang": "de"}], "type": "flow data set", "refObjectId": "a2b32f97-3fc7-4af2-b209-525bc6426f33", "uri": "../flows/a2b32f97-3fc7-4af2-b209-525bc6426f33.xml"}, "exchange direction": "OUTPUT", "other": {"anies": [{"name": "referenceToUnitGroupDataSet", "value": {"shortDescription": [{"value": "kg", "lang": "en"}], "type": "unit group data set", "refObjectId": "ad38d542-3fe9-439d-9b95-2f5f7752acaf", "uri": "../unitgroups/ad38d542-3fe9-439d-9b95-2f5f7752acaf.xml"}}, {"value": "0", "module": "A1-A3"}, {"value": "0", "module": "A4"}, {"value": "0", "module": "A5"}, {"value": "0", "module": "C1"}, {"value": "0", "module": "C2"}, {"value": "0", "module": "C3"}, {"value": "0", "module": "D"}]}, "resolvedFlowVersion": "38.00.000", "flowProperties": [], "typeOfFlow": "Other flow", "classification": {"classHierarchy": "Quantities / Environmental quantities / EPD EN 15804 / LCI indicators", "name": "GaBiCategories"}}, {"dataSetInternalID": 15, "referenceToFlowDataSet": {"shortDescription": [{"value": "Materials for recycling (MFR)", "lang": "en"}, {"value": "Stoffe zum Recycling (MFR)", "lang": "de"}], "type": "flow data set", "refObjectId": "d7fe48a5-4103-49c8-9aae-b0b5dfdbd6ae", "uri": "../flows/d7fe48a5-4103-49c8-9aae-b0b5dfdbd6ae.xml"}, "exchange direction": "OUTPUT", "other": {"anies": [{"name": "referenceToUnitGroupDataSet", "value": {"shortDescription": [{"value": "kg", "lang": "en"}], "type": "unit group data set", "refObjectId": "ad38d542-3fe9-439d-9b95-2f5f7752acaf", "uri": "../unitgroups/ad38d542-3fe9-439d-9b95-2f5f7752acaf.xml"}}, {"value": "0", "module": "A1-A3"}, {"value": "0", "module": "A4"}, {"value": "0", "module": "A5"}, {"value": "0", "module": "C1"}, {"value": "0", "module": "C2"}, {"value": "0", "module": "C3"}, {"value": "0", "module": "D"}]}, "resolvedFlowVersion": "38.00.000", "flowProperties": [], "typeOfFlow": "Other flow", "classification": {"classHierarchy": "Quantities / Environmental quantities / EPD EN 15804 / LCI indicators", "name": "GaBiCategories"}}, {"dataSetInternalID": 16, "referenceToFlowDataSet": {"shortDescription": [{"value": "Materials for energy recovery (MER)", "lang": "en"}, {"value": "Stoffe für die Energierückgewinnung (MER)", "lang": "de"}], "type": "flow data set", "refObjectId": "59a9181c-3aaf-46ee-8b13-2b3723b6e447", "uri": "../flows/59a9181c-3aaf-46ee-8b13-2b3723b6e447.xml"}, "exchange direction": "OUTPUT", "other": {"anies": [{"name": "referenceToUnitGroupDataSet", "value": {"shortDescription": [{"value": "kg", "lang": "en"}], "type": "unit group data set", "refObjectId": "ad38d542-3fe9-439d-9b95-2f5f7752acaf", "uri": "../unitgroups/ad38d542-3fe9-439d-9b95-2f5f7752acaf.xml"}}, {"value": "0", "module": "A1-A3"}, {"value": "0", "module": "A4"}, {"value": "0", "module": "A5"}, {"value": "0", "module": "C1"}, {"value": "0", "module": "C2"}, {"value": "0", "module": "C3"}, {"value": "0", "module": "D"}]}, "resolvedFlowVersion": "38.00.000", "flowProperties": [], "typeOfFlow": "Other flow", "classification": {"classHierarchy": "Quantities / Environmental quantities / EPD EN 15804 / LCI indicators", "name": "GaBiCategories"}}, {"dataSetInternalID": 17, "referenceToFlowDataSet": {"shortDescription": [{"value": "Exported electrical energy (EEE)", "lang": "en"}, {"value": "Exportierte elektrische Energie (EEE)", "lang": "de"}], "type": "flow data set", "refObjectId": "4da0c987-2b76-40d6-9e9e-82a017aaaf29", "uri": "../flows/4da0c987-2b76-40d6-9e9e-82a017aaaf29.xml"}, "exchange direction": "OUTPUT", "other": {"anies": [{"name": "referenceToUnitGroupDataSet", "value": {"shortDescription": [{"value": "MJ", "lang": "en"}], "type": "unit group data set", "refObjectId": "93a60a57-a3c8-11da-a746-0800200c9a66", "uri": "../unitgroups/93a60a57-a3c8-11da-a746-0800200c9a66.xml"}}, {"value": "0", "module": "A1-A3"}, {"value": "0", "module": "A4"}, {"value": "1.244291052", "module": "A5"}, {"value": "0", "module": "C1"}, {"value": "0", "module": "C2"}, {"value": "0", "module": "C3"}, {"value": "0", "module": "D"}]}, "resolvedFlowVersion": "38.00.000", "flowProperties": [], "typeOfFlow": "Other flow", "classification": {"classHierarchy": "Quantities / Environmental quantities / EPD EN 15804 / LCI indicators", "name": "GaBiCategories"}}, {"dataSetInternalID": 18, "referenceToFlowDataSet": {"shortDescription": [{"value": "Exported thermal energy (EET)", "lang": "en"}, {"value": "Exportierte thermische Energie (EET)", "lang": "de"}], "type": "flow data set", "refObjectId": "98daf38a-7a79-46d3-9a37-2b7bd0955810", "uri": "../flows/98daf38a-7a79-46d3-9a37-2b7bd0955810.xml"}, "exchange direction": "OUTPUT", "other": {"anies": [{"name": "referenceToUnitGroupDataSet", "value": {"shortDescription": [{"value": "MJ", "lang": "en"}], "type": "unit group data set", "refObjectId": "93a60a57-a3c8-11da-a746-0800200c9a66", "uri": "../unitgroups/93a60a57-a3c8-11da-a746-0800200c9a66.xml"}}, {"value": "0", "module": "A1-A3"}, {"value": "0", "module": "A4"}, {"value": "2.222169644", "module": "A5"}, {"value": "0", "module": "C1"}, {"value": "0", "module": "C2"}, {"value": "0", "module": "C3"}, {"value": "0", "module": "D"}]}, "resolvedFlowVersion": "38.00.000", "flowProperties": [], "typeOfFlow": "Other flow", "classification": {"classHierarchy": "Quantities / Environmental quantities / EPD EN 15804 / LCI indicators", "name": "GaBiCategories"}}]}, "LCIAResults": {"LCIAResult": [{"referenceToLCIAMethodDataSet": {"shortDescription": [{"value": "Global Warming Potential total (GWP-total)", "lang": "en"}, {"value": "Globales Erwärmungspotenzial total (GWP-total)", "lang": "de"}], "type": "LCIA method data set", "refObjectId": "6a37f984-a4b3-458a-a20a-64418c145fa2", "uri": "../lciamethods/6a37f984-a4b3-458a-a20a-64418c145fa2.xml"}, "other": {"anies": [{"name": "referenceToUnitGroupDataSet", "value": {"shortDescription": [{"value": "kg CO_(2) eq", "lang": "en"}], "type": "unit group data set", "refObjectId": "1ebf3012-d0db-4de2-aefd-ef30cedb0be1", "uri": "../unitgroups/1ebf3012-d0db-4de2-aefd-ef30cedb0be1.xml"}}, {"value": "5.305325682175", "module": "A1-A3"}, {"value": "0.05871720246", "module": "A4"}, {"value": "0.675979556", "module": "A5"}, {"value": "0.0002786595379", "module": "C1"}, {"value": "0.01237939877", "module": "C2"}, {"value": "0.9445000237", "module": "C3"}, {"value": "-0.6251110041", "module": "D"}]}}, {"referenceToLCIAMethodDataSet": {"shortDescription": [{"value": "Global Warming Potential fossil fuels (GWP-fossil)", "lang": "en"}, {"value": "Globales Erwärmungspotenzial fossil (GWP-fossil)", "lang": "de"}], "type": "LCIA method data set", "refObjectId": "5f635281-343e-44fb-83df-1971b155e6b6", "uri": "../lciamethods/5f635281-343e-44fb-83df-1971b155e6b6.xml"}, "other": {"anies": [{"name": "referenceToUnitGroupDataSet", "value": {"shortDescription": [{"value": "kg CO_(2) eq", "lang": "en"}], "type": "unit group data set", "refObjectId": "1ebf3012-d0db-4de2-aefd-ef30cedb0be1", "uri": "../unitgroups/1ebf3012-d0db-4de2-aefd-ef30cedb0be1.xml"}}, {"value": "5.358958440472", "module": "A1-A3"}, {"value": "0.05807747519", "module": "A4"}, {"value": "0.5610055144", "module": "A5"}, {"value": "0.0002662982543", "module": "C1"}, {"value": "0.01183684636", "module": "C2"}, {"value": "0.4292688031", "module": "C3"}, {"value": "-0.6232704822", "module": "D"}]}}, {"referenceToLCIAMethodDataSet": {"shortDescription": [{"value": "Global Warming Potential biogenic (GWP-biogenic)", "lang": "en"}, {"value": "Globales Erwärmungspotenzial biogen (GWP-biogenic)", "lang": "de"}], "type": "LCIA method data set", "refObjectId": "2356e1ab-0185-4db5-86e5-16de51c7485c", "uri": "../lciamethods/2356e1ab-0185-4db5-86e5-16de51c7485c.xml"}, "other": {"anies": [{"name": "referenceToUnitGroupDataSet", "value": {"shortDescription": [{"value": "kg CO_(2) eq", "lang": "en"}], "type": "unit group data set", "refObjectId": "1ebf3012-d0db-4de2-aefd-ef30cedb0be1", "uri": "../unitgroups/1ebf3012-d0db-4de2-aefd-ef30cedb0be1.xml"}}, {"value": "-0.0589167643022", "module": "A1-A3"}, {"value": "0.0001695218598", "module": "A4"}, {"value": "0.1149168883", "module": "A5"}, {"value": "1.235488869E-05", "module": "C1"}, {"value": "0.0005422731999", "module": "C2"}, {"value": "0.5151962379", "module": "C3"}, {"value": "-0.001429919389", "module": "D"}]}}, {"referenceToLCIAMethodDataSet": {"shortDescription": [{"value": "Global Warming Potential luluc (GWP-luluc)", "lang": "en"}, {"value": "Globales Erwärmungspotenzial luluc (GWP-luluc)", "lang": "de"}], "type": "LCIA method data set", "refObjectId": "4331bbdb-978a-490d-8707-eeb047f01a55", "uri": "../lciamethods/4331bbdb-978a-490d-8707-eeb047f01a55.xml"}, "other": {"anies": [{"name": "referenceToUnitGroupDataSet", "value": {"shortDescription": [{"value": "kg CO_(2) eq", "lang": "en"}], "type": "unit group data set", "refObjectId": "1ebf3012-d0db-4de2-aefd-ef30cedb0be1", "uri": "../unitgroups/1ebf3012-d0db-4de2-aefd-ef30cedb0be1.xml"}}, {"value": "0.0052840060295699", "module": "A1-A3"}, {"value": "0.000470205403", "module": "A4"}, {"value": "5.715335632E-05", "module": "A5"}, {"value": "6.394911664E-09", "module": "C1"}, {"value": "2.792066923E-07", "module": "C2"}, {"value": "3.498257312E-05", "module": "C3"}, {"value": "-0.0004106025676", "module": "D"}]}}, {"referenceToLCIAMethodDataSet": {"shortDescription": [{"value": "Depletion potential of the stratospheric ozone layer (ODP)", "lang": "en"}, {"value": "Abbau Potential der stratosphärischen Ozonschicht (ODP)", "lang": "de"}], "type": "LCIA method data set", "refObjectId": "b5c629d6-def3-11e6-bf01-fe55135034f3", "uri": "../lciamethods/b5c629d6-def3-11e6-bf01-fe55135034f3.xml"}, "other": {"anies": [{"name": "referenceToUnitGroupDataSet", "value": {"shortDescription": [{"value": "kg CFC11 eq", "lang": "en"}], "type": "unit group data set", "refObjectId": "d9e957c9-7309-4474-bf3a-7777df6c4e5b", "uri": "../unitgroups/d9e957c9-7309-4474-bf3a-7777df6c4e5b.xml"}}, {"value": "1.99129196508E-13", "module": "A1-A3"}, {"value": "6.979845494E-18", "module": "A4"}, {"value": "2.044262532E-15", "module": "A5"}, {"value": "2.836585201E-20", "module": "C1"}, {"value": "1.238474608E-18", "module": "C2"}, {"value": "3.022187215E-16", "module": "C3"}, {"value": "-6.106848783E-15", "module": "D"}]}}, {"referenceToLCIAMethodDataSet": {"shortDescription": [{"value": "Acidification potential of land and water (AP)", "lang": "en"}, {"value": "Versauerungspotenzial von Boden und Wasser (AP)", "lang": "de"}], "type": "LCIA method data set", "refObjectId": "b5c611c6-def3-11e6-bf01-fe55135034f3", "uri": "../lciamethods/b5c611c6-def3-11e6-bf01-fe55135034f3.xml"}, "other": {"anies": [{"name": "referenceToUnitGroupDataSet", "value": {"shortDescription": [{"value": "mol H^(+) eq", "lang": "en"}], "type": "unit group data set", "refObjectId": "42e089ac-92bf-4bf2-8ca1-5fc40d18f2ed", "uri": "../unitgroups/42e089ac-92bf-4bf2-8ca1-5fc40d18f2ed.xml"}}, {"value": "0.01610709559237", "module": "A1-A3"}, {"value": "0.0001740460232", "module": "A4"}, {"value": "0.0002357578844", "module": "A5"}, {"value": "3.603487497E-06", "module": "C1"}, {"value": "3.734022818E-05", "module": "C2"}, {"value": "0.0005251343523", "module": "C3"}, {"value": "-0.0008449547303", "module": "D"}]}}, {"referenceToLCIAMethodDataSet": {"shortDescription": [{"value": "Eutrophication potential aquatic freshwater (EP-freshwater)", "lang": "en"}, {"value": "Eutrophierungspotenzial Süßwasser (EP-freshwater)", "lang": "de"}], "type": "LCIA method data set", "refObjectId": "b53ec18f-7377-4ad3-86eb-cc3f4f276b2b", "uri": "../lciamethods/b53ec18f-7377-4ad3-86eb-cc3f4f276b2b.xml"}, "other": {"anies": [{"name": "referenceToUnitGroupDataSet", "value": {"shortDescription": [{"value": "kg P eq", "lang": "en"}], "type": "unit group data set", "refObjectId": "0429039d-a61d-4590-ba67-aa4a20a810a1", "uri": "../unitgroups/0429039d-a61d-4590-ba67-aa4a20a810a1.xml"}}, {"value": "9.351437238204E-06", "module": "A1-A3"}, {"value": "1.765141825E-07", "module": "A4"}, {"value": "1.020263311E-07", "module": "A5"}, {"value": "5.750761277E-11", "module": "C1"}, {"value": "2.51082598E-09", "module": "C2"}, {"value": "1.035728106E-07", "module": "C3"}, {"value": "-7.560829715E-07", "module": "D"}]}}, {"referenceToLCIAMethodDataSet": {"shortDescription": [{"value": "Eutrophication potential aquatic marine (EP-marine)", "lang": "en"}, {"value": "Eutrophierungspotenzial Salzwasser (EP-marine)", "lang": "de"}], "type": "LCIA method data set", "refObjectId": "b5c619fa-def3-11e6-bf01-fe55135034f3", "uri": "../lciamethods/b5c619fa-def3-11e6-bf01-fe55135034f3.xml"}, "other": {"anies": [{"name": "referenceToUnitGroupDataSet", "value": {"shortDescription": [{"value": "kg N eq", "lang": "en"}], "type": "unit group data set", "refObjectId": "d05bb823-ecdf-4686-8c40-bf1d9257859f", "uri": "../unitgroups/d05bb823-ecdf-4686-8c40-bf1d9257859f.xml"}}, {"value": "0.003596080058279", "module": "A1-A3"}, {"value": "7.75136912E-05", "module": "A4"}, {"value": "5.487754977E-05", "module": "A5"}, {"value": "1.634488904E-06", "module": "C1"}, {"value": "1.715462097E-05", "module": "C2"}, {"value": "0.000200798198", "module": "C3"}, {"value": "-0.0002213079585", "module": "D"}]}}, {"referenceToLCIAMethodDataSet": {"shortDescription": [{"value": "Eutrophication potential terrestrial (EP-terrestrial)", "lang": "en"}, {"value": "Eutrophierungspotenzial Land (EP-terrestrial)", "lang": "de"}], "type": "LCIA method data set", "refObjectId": "b5c614d2-def3-11e6-bf01-fe55135034f3", "uri": "../lciamethods/b5c614d2-def3-11e6-bf01-fe55135034f3.xml"}, "other": {"anies": [{"name": "referenceToUnitGroupDataSet", "value": {"shortDescription": [{"value": "mol N eq", "lang": "en"}], "type": "unit group data set", "refObjectId": "71b4d617-0ec9-4d3f-b65e-e438940c2401", "uri": "../unitgroups/71b4d617-0ec9-4d3f-b65e-e438940c2401.xml"}}, {"value": "0.03918693666791", "module": "A1-A3"}, {"value": "0.0008681454276", "module": "A4"}, {"value": "0.000740010324", "module": "A5"}, {"value": "1.790057665E-05", "module": "C1"}, {"value": "0.0001888277157", "module": "C2"}, {"value": "0.002523199766", "module": "C3"}, {"value": "-0.002374863108", "module": "D"}]}}, {"referenceToLCIAMethodDataSet": {"shortDescription": [{"value": "Formation potential of tropospheric ozone photochemical oxidants (POCP)", "lang": "en"}, {"value": "Bildungspotential für troposphärisches Ozon (POCP)", "lang": "de"}], "type": "LCIA method data set", "refObjectId": "b5c610fe-def3-11e6-bf01-fe55135034f3", "uri": "../lciamethods/b5c610fe-def3-11e6-bf01-fe55135034f3.xml"}, "other": {"anies": [{"name": "referenceToUnitGroupDataSet", "value": {"shortDescription": [{"value": "kg NMVOC eq", "lang": "en"}], "type": "unit group data set", "refObjectId": "d27c25f8-fbc1-44c6-b47b-4adbae4199c6", "uri": "../unitgroups/d27c25f8-fbc1-44c6-b47b-4adbae4199c6.xml"}}, {"value": "0.01432235688938", "module": "A1-A3"}, {"value": "0.0001531704875", "module": "A4"}, {"value": "0.009637001749", "module": "A5"}, {"value": "4.912404435E-06", "module": "C1"}, {"value": "3.387688189E-05", "module": "C2"}, {"value": "0.0005215223476", "module": "C3"}, {"value": "-0.0006381757127", "module": "D"}]}}, {"referenceToLCIAMethodDataSet": {"shortDescription": [{"value": "Abiotic depletion potential for non fossil resources (ADPE)", "lang": "en"}, {"value": "Potenzial für den abiotischen Abbau nicht fossiler Ressourcen (ADPE)", "lang": "de"}], "type": "LCIA method data set", "refObjectId": "b2ad6494-c78d-11e6-9d9d-cec0c932ce01", "uri": "../lciamethods/b2ad6494-c78d-11e6-9d9d-cec0c932ce01.xml"}, "other": {"anies": [{"name": "referenceToUnitGroupDataSet", "value": {"shortDescription": [{"value": "kg Sb eq", "lang": "en"}], "type": "unit group data set", "refObjectId": "54ccd2d9-a32a-4fc2-923d-f2c8c93e89d4", "uri": "../unitgroups/54ccd2d9-a32a-4fc2-923d-f2c8c93e89d4.xml"}}, {"value": "0.000108647130454835", "module": "A1-A3"}, {"value": "4.163682369E-09", "module": "A4"}, {"value": "1.087307795E-06", "module": "A5"}, {"value": "8.058691308E-12", "module": "C1"}, {"value": "3.518485732E-10", "module": "C2"}, {"value": "4.615294113E-09", "module": "C3"}, {"value": "-9.798741474E-08", "module": "D"}]}}, {"referenceToLCIAMethodDataSet": {"shortDescription": [{"value": "Abiotic depletion potential for fossil resources (ADPF)", "lang": "en"}, {"value": "Potenzial für den abiotischen Abbau fossiler Brennstoffe (ADPF)", "lang": "de"}], "type": "LCIA method data set", "refObjectId": "b2ad6110-c78d-11e6-9d9d-cec0c932ce01", "uri": "../lciamethods/b2ad6110-c78d-11e6-9d9d-cec0c932ce01.xml"}, "other": {"anies": [{"name": "referenceToUnitGroupDataSet", "value": {"shortDescription": [{"value": "MJ", "lang": "en"}], "type": "unit group data set", "refObjectId": "93a60a57-a3c8-11da-a746-0800200c9a66", "uri": "../unitgroups/93a60a57-a3c8-11da-a746-0800200c9a66.xml"}}, {"value": "97.87123975271", "module": "A1-A3"}, {"value": "0.7731417236", "module": "A4"}, {"value": "1.07133459", "module": "A5"}, {"value": "0.003810342929", "module": "C1"}, {"value": "0.1663624615", "module": "C2"}, {"value": "0.5521597506", "module": "C3"}, {"value": "-10.5504855", "module": "D"}]}}, {"referenceToLCIAMethodDataSet": {"shortDescription": [{"value": "Water use (WDP)", "lang": "en"}, {"value": "Wassernutzung (WDP)", "lang": "de"}], "type": "LCIA method data set", "refObjectId": "b2ad66ce-c78d-11e6-9d9d-cec0c932ce01", "uri": "../lciamethods/b2ad66ce-c78d-11e6-9d9d-cec0c932ce01.xml"}, "other": {"anies": [{"name": "referenceToUnitGroupDataSet", "value": {"shortDescription": [{"value": "m^(3) world eq deprived", "lang": "en"}], "type": "unit group data set", "refObjectId": "6ae2df01-888e-46c8-b17d-49fa3869b476", "uri": "../unitgroups/6ae2df01-888e-46c8-b17d-49fa3869b476.xml"}}, {"value": "1.66567677432335", "module": "A1-A3"}, {"value": "0.0005190876595", "module": "A4"}, {"value": "0.07648185214", "module": "A5"}, {"value": "5.26510258E-07", "module": "C1"}, {"value": "2.29878371E-05", "module": "C2"}, {"value": "0.1568875378", "module": "C3"}, {"value": "-0.06065727519", "module": "D"}]}}, {"referenceToLCIAMethodDataSet": {"shortDescription": [{"value": "Incidence of disease due to PM emissions (PM)", "lang": "en"}, {"value": "Auftreten von Krankheiten aufgrund von Feinstaubemissionen (PM)", "lang": "de"}], "type": "LCIA method data set", "refObjectId": "b5c602c6-def3-11e6-bf01-fe55135034f3", "uri": "../lciamethods/b5c602c6-def3-11e6-bf01-fe55135034f3.xml"}, "other": {"anies": [{"name": "referenceToUnitGroupDataSet", "value": {"shortDescription": [{"value": "Disease incidence", "lang": "en"}], "type": "unit group data set", "refObjectId": "3883559b-648f-4afc-8ba2-0bd24f3affa3", "uri": "../unitgroups/3883559b-648f-4afc-8ba2-0bd24f3affa3.xml"}}, {"module": "A1-A3"}, {"module": "A4"}, {"module": "A5"}, {"module": "C1"}, {"module": "C2"}, {"module": "C3"}, {"module": "D"}]}}, {"referenceToLCIAMethodDataSet": {"shortDescription": [{"value": "Human exposure efficiency relative to U235 (IR)", "lang": "en"}, {"value": "Wirkung durch Exposition des Menschen mit U235 (IR)", "lang": "de"}], "type": "LCIA method data set", "refObjectId": "b5c632be-def3-11e6-bf01-fe55135034f3", "uri": "../lciamethods/b5c632be-def3-11e6-bf01-fe55135034f3.xml"}, "other": {"anies": [{"name": "referenceToUnitGroupDataSet", "value": {"shortDescription": [{"value": "kBq U235 eq", "lang": "en"}], "type": "unit group data set", "refObjectId": "456b05bf-1415-44a9-9993-02452f554c09", "uri": "../unitgroups/456b05bf-1415-44a9-9993-02452f554c09.xml"}}, {"module": "A1-A3"}, {"module": "A4"}, {"module": "A5"}, {"module": "C1"}, {"module": "C2"}, {"module": "C3"}, {"module": "D"}]}}, {"referenceToLCIAMethodDataSet": {"shortDescription": [{"value": "Comparative toxic unit for ecosystems (ETP-fw)", "lang": "en"}, {"value": "Toxizitätsvergleichseinheit für Ökosysteme (ETP-fw)", "lang": "de"}], "type": "LCIA method data set", "refObjectId": "ee1082d1-b0f7-43ca-a1f0-21e2a4a74511", "uri": "../lciamethods/ee1082d1-b0f7-43ca-a1f0-21e2a4a74511.xml"}, "other": {"anies": [{"name": "referenceToUnitGroupDataSet", "value": {"shortDescription": [{"value": "CTUe", "lang": "en"}], "type": "unit group data set", "refObjectId": "aa959ded-f1eb-4efb-9c5c-2d60be36b3e6", "uri": "../unitgroups/aa959ded-f1eb-4efb-9c5c-2d60be36b3e6.xml"}}, {"module": "A1-A3"}, {"module": "A4"}, {"module": "A5"}, {"module": "C1"}, {"module": "C2"}, {"module": "C3"}, {"module": "D"}]}}, {"referenceToLCIAMethodDataSet": {"shortDescription": [{"value": "Comparative toxic unit for humans (carcinogenic) (HTP-c)", "lang": "en"}, {"value": "Toxizitätsvergleichseinheit für Menschen (krebserregend) (HTP-c)", "lang": "de"}], "type": "LCIA method data set", "refObjectId": "2299222a-bbd8-474f-9d4f-4dd1f18aea7c", "uri": "../lciamethods/2299222a-bbd8-474f-9d4f-4dd1f18aea7c.xml"}, "other": {"anies": [{"name": "referenceToUnitGroupDataSet", "value": {"shortDescription": [{"value": "CTUh", "lang": "en"}], "type": "unit group data set", "refObjectId": "d4c9523e-2d7e-49fd-8469-998f547d3a70", "uri": "../unitgroups/d4c9523e-2d7e-49fd-8469-998f547d3a70.xml"}}, {"module": "A1-A3"}, {"module": "A4"}, {"module": "A5"}, {"module": "C1"}, {"module": "C2"}, {"module": "C3"}, {"module": "D"}]}}, {"referenceToLCIAMethodDataSet": {"shortDescription": [{"value": "Comparative toxic unit for humans (noncarcinogenic) (HTP-nc)", "lang": "en"}, {"value": "Toxizitätsvergleichseinheit für Menschen (nicht krebserregend) (HTP-nc)", "lang": "de"}], "type": "LCIA method data set", "refObjectId": "3af763a5-b7a1-48c9-9cee-1f223481fcef", "uri": "../lciamethods/3af763a5-b7a1-48c9-9cee-1f223481fcef.xml"}, "other": {"anies": [{"name": "referenceToUnitGroupDataSet", "value": {"shortDescription": [{"value": "CTUh", "lang": "en"}], "type": "unit group data set", "refObjectId": "d4c9523e-2d7e-49fd-8469-998f547d3a70", "uri": "../unitgroups/d4c9523e-2d7e-49fd-8469-998f547d3a70.xml"}}, {"module": "A1-A3"}, {"module": "A4"}, {"module": "A5"}, {"module": "C1"}, {"module": "C2"}, {"module": "C3"}, {"module": "D"}]}}, {"referenceToLCIAMethodDataSet": {"shortDescription": [{"value": "Soil quality index (SQP)", "lang": "en"}, {"value": "Bodenqualitätsindex (SQP)", "lang": "de"}], "type": "LCIA method data set", "refObjectId": "b2ad6890-c78d-11e6-9d9d-cec0c932ce01", "uri": "../lciamethods/b2ad6890-c78d-11e6-9d9d-cec0c932ce01.xml"}, "other": {"anies": [{"name": "referenceToUnitGroupDataSet", "value": {"shortDescription": [{"value": "SQP", "lang": "en"}], "type": "unit group data set", "refObjectId": "f130951c-e67f-4f7f-8dd4-665de3974e18", "uri": "../unitgroups/f130951c-e67f-4f7f-8dd4-665de3974e18.xml"}}, {"module": "A1-A3"}, {"module": "A4"}, {"module": "A5"}, {"module": "C1"}, {"module": "C2"}, {"module": "C3"}, {"module": "D"}]}}]}, "otherAttributes": {"{http://www.indata.network/EPD/2019}epd-version": "1.2"}, "version": "1.1", "locations": "../ILCDLocations.xml"}