{"processInformation": {"dataSetInformation": {"UUID": "cf69cb37-552b-492d-a9a0-1d4e28b0bf95", "name": {"baseName": [{"value": "Tufted carpet tiles with 100% recycled PA6 pile material and bitumen-based heavy backing, LC2", "lang": "en"}, {"value": "Getuftete Teppichfliesen mit 100% recyceltem PA6-Flormaterial und schwerem Rücken auf Bitumenbasis, LC2", "lang": "de"}], "functionalUnitFlowProperties": [{"lang": "en"}]}, "classificationInformation": {"classification": [{"class": [{"value": "Kunststoffe", "level": 0, "classId": "6"}, {"value": "Bodenbeläge", "level": 1, "classId": "6.2"}, {"value": "Textile Bodenbeläge", "level": 2, "classId": "6.2.05"}], "name": "OEKOBAU.DAT"}, {"class": [{"value": "02 Building products", "level": 0}, {"value": "Floor coverings", "level": 1}, {"value": "Floor coverings", "level": 2}], "name": "IBUCategories"}]}, "generalComment": [{"value": "The declaration applies to tufted carpet tiles having a pile material of polyamide 6 with 100% recycled content and a bitumen-based heavy backing with a maximum weight of 3200 g/m2. The total recycled content of the carpet is 17%. The products correspond to luxury class LC2 with a limitation of the maximum surface pile weight of 600 g/m and a maximum total pile weight of 850 g/m2.Colouring and design of the use layer may be achieved by aqueous dyeing methods or by using solution-dyed yarns.", "lang": "en"}, {"value": "Die Deklaration gilt für getuftete Teppichfliesen mit einem Polmaterial aus Polyamid 6 mit 100% recyceltem Anteil und einem schweren Rücken auf Bitumenbasis mit einem Höchstgewicht von 3200 g/m2. Der Gesamtgehalt des Teppichs an recyceltem Material beträgt 17%. Die Produkte entsprechen der Luxusklasse LC2 mit einer Beschränkung auf ein maximales Flächenpolgewicht von 600 g/m² und ein maximales Gesamtpolgewicht von 850 g/m2. Die Färbung und das Design der Nutzschicht können durch wässrige Färbemethoden oder durch die Verwendung von lösungsgefärbten Garnen erreicht werden.", "lang": "de"}], "other": {"anies": [{"scenario": [{"description": [{"value": "Deponie", "lang": "en"}, {"value": "Deponie", "lang": "de"}], "name": "S1", "default": true}, {"description": [{"value": "MVA", "lang": "en"}, {"value": "MVA", "lang": "de"}], "name": "S2"}, {"description": [{"value": "Zementwerk", "lang": "en"}, {"value": "Zementwerk", "lang": "de"}], "name": "S3"}]}]}}, "quantitativeReference": {"referenceToReferenceFlow": [0]}, "time": {"referenceYear": 2023, "dataSetValidUntil": 2028, "other": {"anies": [{"name": "publicationDateOfEPD", "value": 1692576000000}]}}, "geography": {"locationOfOperationSupplyOrProduction": {"location": "RER"}}, "technology": {"technologyDescriptionAndIncludedProcesses": [{"value": "Tufted carpet tiles having a pile material of polyamide 6 with 100% recycled content and a bitumen-based heavy backing. \nTechnical data: \nThe technical data describes a fictitious worst-case product representing all products with the described characteristics.", "lang": "en"}, {"value": "Getuftete Teppichfliesen mit einem Polmaterial aus Polyamid 6 mit 100% recyceltem Anteil und einem schweren Rücken auf Bitumenbasis. \nTechnische Daten: \nDie technischen Daten beschreiben ein fiktives Worst-Case-Produkt, das für alle Produkte mit den beschriebenen Eigenschaften steht. \nDeklarierte Einheit: \nDie angegebene Einheit bezieht sich auf 1 m²  produzierten textilen Bodenbelag. Der Output von Modul A5 \"Montage\" ist 1 m² verlegter textiler Bodenbelag. Die Rohdichte beträgt 600 kg/m².\n", "lang": "de"}], "technologicalApplicability": [{"value": "The use class of the specific product as defined in EN 1307 can be found in the Product Information System (PRODIS) using the PRODIS registration number of the product.", "lang": "en"}, {"value": "Die in der EN 1307 definierte Verwendungsklasse des jeweiligen Produkts finden Sie im Produktinformationssystem (PRODIS) unter Verwendung der PRODIS-Registrierungsnummer des Produkts.", "lang": "de"}]}}, "modellingAndValidation": {"LCIMethodAndAllocation": {"typeOfDataSet": "EPD", "referenceToLCAMethodDetails": [{"shortDescription": [{"value": "Floor coverings.pdf", "lang": "en"}], "type": "source data set", "refObjectId": "5f357b17-32f3-4318-8df7-3106db276bd3"}], "other": {"anies": [{"name": "subType", "value": "representative dataset"}]}}, "dataSourcesTreatmentAndRepresentativeness": {"referenceToDataSource": [{"shortDescription": [{"value": "GaBi Database (all versions)", "lang": "en"}], "type": "source data set", "refObjectId": "28d74cc0-db8b-4d7e-bc44-5f6d56ce0c4a"}, {"shortDescription": [{"value": "GaBi Database Edition 2022, CUP 2022.02", "lang": "en"}], "type": "source data set", "refObjectId": "94f442cb-662e-43ea-a792-4b0a35132e93"}], "useAdviceForDataSet": [{"value": "Scope: \nThis sample EPD applies to all products of the member companies of the Gemeinschaft umweltfreundlicher Teppichboden (GUT) e.V. that comply with the product descriptions and are registered in the GUT/PRODIS information system. It is only valid in conjunction with a valid GUT/PRODIS license of the product.\nThe construction and production data of the registered products are provided by the member companies of the GUT e.V.. The production sites are located in Belgium, France, Germany, Great Britain, Ireland and The Netherlands. \nSystem boundary: \nType of EPD:\nCradle-to-gate with options, module C1-C4, module D, and additional modules A4, A5, B1, B2.\n\nSystem boundaries of modules A, B, C, D:\nModules C3, C4 and D are indicated separately for three end-of-life scenarios:\n1 - landfill disposal\n2 - municipal waste incineration\n3 - recovery in a cement plant\n\nA1-A3 Production:\nEnergy supply and production of the basic material, processing of secondary material, auxiliary material, transport of the material to the manufacturing site, emissions, waste water treatment, packaging material and waste processing up to the landfill disposal of residual waste (except radioactive waste). Potential benefits for generated electricity and steam due to the incineration of production waste are aggregated. Biogenic carbon that is stored in renewable material (packaging paper) is taken into account as well as the associated carbon dioxide uptake from the air from which this biogenic carbon comes.\n\nA4 Transport:\nTransport of the packed textile floor covering from factory gate to the place of installation.\n\nA5 Installation:\nInstallation of the textile floor covering, processing of installation waste and packaging waste up to the landfill disposal of residual waste (except radioactive waste), the production of the amount of carpet that occurs as installation waste including its transport to the place of installation. Generated electricity and steam due to the incineration of waste are listed in the result table as exported energy. Biogenic carbon that is stored in renewable materials in packaging paper is released as carbon dioxide emissions into the air at the end of life in module A5. Preparation of the floor and auxiliary materials (adhesives, fixing agents, PET connectors) are beyond the system boundaries and not taken into account.\n\nB1 Use:\nIndoor emissions during the use stage. After the first year, no product-related Volatile Organic Compound (VOC) emissions are relevant due to known VOC decay curves of the product.\n\nB2 Maintenance:\nCleaning of the textile floor covering for a period of 1 year:\nVacuum cleaning – electricity supply\nWet cleaning – electricity, water consumption, production of the cleaning agent, waste water treatment. The declared values in this module have to be multiplied by the assumed service life of the floor covering in the building in question.\n\nB3 - B5:\nThe modules are not relevant within the assumed reference service life of 10 years.\n\nB6 - B7:\nNo energy and water input are required for the operation of the carpet in the use stage. The modules are not relevant and not declared.\n\nC1 De-construction:\nThe floor covering is de-constructed manually and no additional environmental impact is caused.\n\nC2 Transport:\nTransport of the carpet waste to a landfill, to the municipal waste incineration\nplant (MWI) or to the waste collection facility for recycling.\n\nC3 Waste processing:\nC3-1: Landfill disposal needs no waste processing. \nC3-2: Impact from waste incineration (plant with R1 > 0.6), generated electricity and steam are listed in the result table as exported energy.\nC3-3:\nCollection of the carpet waste for recovery in the cement industry, waste processing (granulating), transport to the cement plant, emissions from the incineration.\n\nC4 Disposal\nC4-1: Impact from landfill disposal,\nC4-2: The carpet waste leaves the system in \nmodule C3-2,\nC4-3: The pre-processed carpet waste leaves the system in module C3-3.\n\nD Recycling potential:\nCalculated potential benefits result from materials exclusive secondary materials (net materials).\nD-A5: Potential benefits for generated energy due to incineration of packaging and installation waste (incineration plant with R1 > 0.6), \nD-1: Potential benefits for generated energy due to landfill disposal of carpet waste at the end of life,\nD-2: Potential benefits for generated energy due to incineration of carpet waste at the end-of life (incineration plant with R1 > 0.6),\nD-3: Potential benefits for saved fossil energy and saved inorganic material due to recovery of the carpet in a cement plant.", "lang": "en"}, {"value": "Gültigkeitsbereich: \nDiese Muster-EPD gilt für alle Produkte der Mitgliedsunternehmen der Gemeinschaft umweltfreundlicher Teppichboden (GUT) e.V., die den Produktbeschreibungen entsprechen und im Informationssystem GUT/PRODIS registriert sind. Sie ist nur in Verbindung mit einer gültigen GUT/PRODIS-Lizenz des Produkts gültig. Die Konstruktions- und Produktionsdaten der registrierten Produkte werden von den Mitgliedsunternehmen der GUT e.V. bereitgestellt. Die Produktionsstätten befinden sich in Belgien, Frankreich, Deutschland, Großbritannien, Irland und den Niederlanden. \nSystemgrenze: \nArt der EPD: Cradle-to-Gate mit Optionen, Modul C1-C4, Modul D und zusätzliche Module A4, A5, B1, B2.\n\nSystemgrenzen der Module A, B, C, D: Die Module C3, C4 und D sind separat für drei End-of-Life-Szenarien angegeben: 1 - Deponierung 2 - Verbrennung von Siedlungsabfällen 3 - Verwertung in einem Zementwerk A1-A3 Produktion: Energieversorgung und Produktion des Ausgangsmaterials, Verarbeitung von Sekundärmaterial, Hilfsstoffen, Transport des Materials zur Produktionsstätte, Emissionen, Abwasserbehandlung, Verpackungsmaterial und Abfallverarbeitung bis hin zur Deponierung von Restmüll (außer radioaktivem Abfall). Potenzielle Vorteile für die Erzeugung von Strom und Dampf durch die Verbrennung von Produktionsabfällen werden zusammengerechnet. Biogener Kohlenstoff, der in erneuerbarem Material (Verpackungspapier) gespeichert ist, wird ebenso berücksichtigt wie die damit verbundene Kohlendioxidaufnahme aus der Luft, aus der dieser biogene Kohlenstoff stammt. A4 Transport: Transport des verpackten textilen Bodenbelags vom Werkstor zum Verlegeort. A5 Verlegung: Verlegung des textilen Bodenbelags, Verarbeitung von Verlegeabfällen und Verpackungsabfällen bis zur Deponierung von Restmüll (außer radioaktiven Abfällen), die Produktion der als Verlegeabfall anfallenden Teppichmenge einschließlich ihres Transports zum Verlegeort. Die durch die Verbrennung von Abfällen erzeugte Elektrizität und Dampf werden in der Ergebnistabelle als exportierte Energie aufgeführt. Biogener Kohlenstoff, der in erneuerbaren Materialien in Verpackungspapier gespeichert ist, wird am Ende der Lebensdauer in Modul A5 als Kohlendioxidemissionen in die Luft abgegeben. Die Vorbereitung des Bodens und die Hilfsmaterialien (Klebstoffe, Befestigungsmittel, PET-Verbindungsstücke) liegen außerhalb der Systemgrenzen und werden nicht berücksichtigt. B1 Nutzung: Emissionen in Innenräumen während der Nutzungsphase. Nach dem ersten Jahr sind aufgrund der bekannten VOC-Zerfallskurven des Produkts keine produktbezogenen Emissionen flüchtiger organischer Verbindungen (VOC) relevant. B2 Pflege: Reinigung des textilen Bodenbelags für einen Zeitraum von 1 Jahr: Staubsaugen - Stromzufuhr Nassreinigung - Strom, Wasserverbrauch, Herstellung des Reinigungsmittels, Abwasseraufbereitung. Die deklarierten Werte in diesem Modul müssen mit der angenommenen Nutzungsdauer des Bodenbelags in dem betreffenden Gebäude multipliziert werden. B3 - B5: Die Module sind innerhalb der angenommenen Referenznutzungsdauer von 10 Jahren nicht relevant. B6 - B7: Für den Betrieb des Teppichbodens in der Nutzungsphase ist kein Energie- und Wassereinsatz erforderlich. Die Module sind nicht relevant und werden nicht deklariert. C1 Rückbau: Der Rückbau des Bodenbelags erfolgt manuell und verursacht keine zusätzlichen Umweltauswirkungen. C2 Transport: Transport des Teppichabfalls zu einer Deponie, zur kommunalen Müllverbrennungsanlage (KVA) oder zur Abfallsammelstelle für das Recycling. C3 Abfallverarbeitung: C3-1: Die Deponierung erfordert keine Abfallverarbeitung. \nC3-2: Auswirkungen der Abfallverbrennung (Anlage mit R1 > 0,6), erzeugter Strom und Dampf werden in der Ergebnistabelle als exportierte Energie aufgeführt. C3-3: Sammlung der Teppichabfälle zur Verwertung in der Zementindustrie, Abfallverarbeitung (Granulieren), Transport zum Zementwerk, Emissionen aus der Verbrennung.\n\nC4 Entsorgung C4-1: Auswirkung der Deponierung, C4-2: Der Teppichabfall verlässt das System in Modul C3-2, C4-3: Der vorverarbeitete Teppichabfall verlässt das System in Modul C3-3. D Verwertungspotenzial: Der berechnete potenzielle Nutzen ergibt sich aus den Materialien ausschließlich der Sekundärmaterialien (Nettomaterialien).\nD-A5: Potenzieller Nutzen für erzeugte Energie aufgrund der Verbrennung von Verpackungs- und Installationsabfällen (Verbrennungsanlage mit R1 > 0,6), D-1: Potenzieller Nutzen für erzeugte Energie aufgrund der Deponierung von Teppichabfällen am Ende der Lebensdauer, D-2: Potenzieller Nutzen für erzeugte Energie aufgrund der Verbrennung von Teppichabfällen am Ende der Lebensdauer (Verbrennungsanlage mit R1 > 0,6), D-3: Potenzieller Nutzen für eingesparte fossile Energie und eingespartes anorganisches Material aufgrund der Verwertung des Teppichs in einem Zementwerk.", "lang": "de"}], "other": {"anies": [{"name": "referenceToOriginalEPD", "value": {"shortDescription": {"value": "Tufted carpet tiles with 100% recycled PA6 pile material and bitumen-based heavy backing, LC2.pdf", "defaultValue": "Tufted carpet tiles with 100% recycled PA6 pile material and bitumen-based heavy backing, LC2.pdf", "lstrings": [{"lang": "en", "value": "Tufted carpet tiles with 100% recycled PA6 pile material and bitumen-based heavy backing, LC2.pdf"}]}, "type": "source data set", "uuid": {"uuid": "700afd20-b277-416c-9fc3-c6df77a3617f"}, "refObjectId": "700afd20-b277-416c-9fc3-c6df77a3617f", "resourceURLs": ["https://oekobaudat.de/OEKOBAU.DAT/resource/sources/700afd20-b277-416c-9fc3-c6df77a3617f/Tufted_carpet_tiles_with_100_recycled_PA6_pile_material_and_bitumen-based_heavy_backing_LC2_18508.pdf?version=00.01.000"]}}]}}, "validation": {"review": [{"referenceToNameOfReviewerAndInstitution": [{"shortDescription": [{"value": "Institut Bauen und Umwelt e. V.", "lang": "en"}], "type": "contact data set", "refObjectId": "d111dbec-b024-4be5-86c5-752d6eb2cf95", "uri": "../contacts/d111dbec-b024-4be5-86c5-752d6eb2cf95.xml"}], "type": "Accredited third party review"}]}, "complianceDeclarations": {"compliance": [{"referenceToComplianceSystem": {"shortDescription": [{"value": "DIN EN 15804+A2", "lang": "en"}], "type": "source data set", "refObjectId": "c0016b33-8cf7-415c-ac6e-deba0d21440d", "uri": "../sources/c0016b33-8cf7-415c-ac6e-deba0d21440d.xml"}}, {"referenceToComplianceSystem": {"shortDescription": [{"value": "ISO 14025", "lang": "en"}], "type": "source data set", "refObjectId": "4f2eb655-6e44-4874-a95a-e28f5442cd4d", "uri": "../sources/4f2eb655-6e44-4874-a95a-e28f5442cd4d.xml"}}]}}, "administrativeInformation": {"commissionerAndGoal": {"referenceToCommissioner": [{"shortDescription": [{"value": "Gemeinschaft umweltfreundlicher Teppichboden (GUT) e.V.", "lang": "en"}], "type": "contact data set", "refObjectId": "1e593d93-ef5b-4ddc-9b55-f58cf8960f3e", "uri": "../contacts/1e593d93-ef5b-4ddc-9b55-f58cf8960f3e.xml"}]}, "dataGenerator": {"referenceToPersonOrEntityGeneratingTheDataSet": [{"shortDescription": [{"value": "Gemeinschaft umweltfreundlicher Teppichboden (GUT) e.V.", "lang": "en"}], "type": "contact data set", "refObjectId": "1e593d93-ef5b-4ddc-9b55-f58cf8960f3e", "uri": "../contacts/1e593d93-ef5b-4ddc-9b55-f58cf8960f3e.xml"}]}, "dataEntryBy": {"timeStamp": 1692576000000, "referenceToDataSetFormat": [{"shortDescription": [{"value": "ILCD Format", "lang": "en"}], "type": "source data set", "refObjectId": "a97a0155-0234-4b87-b4ce-a45da52f2a40", "uri": "../sources/a97a0155-0234-4b87-b4ce-a45da52f2a40.xml"}, {"shortDescription": [{"value": "EPD-Datenformaterweiterungen v1.2", "lang": "de"}, {"value": "EPD Data Format Extensions v1.2", "lang": "en"}], "type": "source data set", "refObjectId": "a29449fd-aa2f-4de8-b5d7-4b06b43c6fde", "uri": "../sources/a29449fd-aa2f-4de8-b5d7-4b06b43c6fde.xml"}]}, "publicationAndOwnership": {"dataSetVersion": "00.02.000", "referenceToRegistrationAuthority": {"shortDescription": [{"value": "Institut Bauen und Umwelt e. V.", "lang": "en"}], "type": "contact data set", "refObjectId": "d111dbec-b024-4be5-86c5-752d6eb2cf95", "uri": "../contacts/d111dbec-b024-4be5-86c5-752d6eb2cf95.xml"}, "registrationNumber": "EPD-GUT-20220083-CBG2-EN", "referenceToOwnershipOfDataSet": {"shortDescription": [{"value": "Gemeinschaft umweltfreundlicher Teppichboden (GUT) e.V.", "lang": "en"}], "type": "contact data set", "refObjectId": "1e593d93-ef5b-4ddc-9b55-f58cf8960f3e", "uri": "../contacts/1e593d93-ef5b-4ddc-9b55-f58cf8960f3e.xml"}, "copyright": true, "licenseType": "Free of charge for all users and uses", "accessRestrictions": [{"value": "None", "lang": "en"}], "other": {"anies": [{"name": "referenceToPublisher", "value": {"shortDescription": [{"value": "Institut Bauen und Umwelt e. V.", "lang": "en"}], "type": "contact data set", "refObjectId": "d111dbec-b024-4be5-86c5-752d6eb2cf95", "uri": "../contacts/d111dbec-b024-4be5-86c5-752d6eb2cf95.xml"}}]}}}, "exchanges": {"exchange": [{"dataSetInternalID": 0, "referenceToFlowDataSet": {"shortDescription": [{"value": "Tufted carpet tiles with 100% recycled PA6 pile material and bitumen-based heavy backing, LC2 (Getufteter Teppichfliesen mit Bitumenrücken, LC2, Polmaterial 100% rec. PA6)", "lang": "en"}], "type": "flow data set", "refObjectId": "af28dd9a-2b1f-53bd-af65-8ac49225bb2f", "uri": "../flows/af28dd9a-2b1f-53bd-af65-8ac49225bb2f.xml"}, "meanAmount": 1.0, "referencesToDataSource": {}, "referenceFlow": true, "resolvedFlowVersion": "00.02.000", "resultingflowAmount": 1.0, "flowProperties": [{"name": [{"lang": "en", "value": "Area"}, {"lang": "de", "value": "Fläche"}], "uuid": "93a60a56-a3c8-19da-a746-0800200c9a66", "referenceFlowProperty": true, "meanValue": 1.0, "referenceUnit": "qm", "unitGroupUUID": "c20a03d7-bd90-4569-bc94-66cfd364dfc8"}], "materialProperties": [{"name": "gross density", "value": "600.0", "unit": "kg/m^3", "unitDescription": "kilograms per cubic metre"}, {"name": "grammage", "value": "5.0", "unit": "kg/m^2", "unitDescription": "kilograms per square meter"}, {"name": "layer thickness", "value": "0.008", "unit": "m", "unitDescription": "meters"}], "typeOfFlow": "Product flow", "classification": {"classHierarchy": "Kunststoffe / Bodenbeläge / Textile Bodenbeläge", "name": "OEKOBAU.DAT"}}, {"dataSetInternalID": 1, "referenceToFlowDataSet": {"shortDescription": [{"value": "Renewable primary energy as energy carrier (PERE)", "lang": "en"}, {"value": "Erneuerbare Primärenergie als Energieträger (PERE)", "lang": "de"}], "type": "flow data set", "refObjectId": "20f32be5-0398-4288-9b6d-accddd195317", "uri": "../flows/20f32be5-0398-4288-9b6d-accddd195317.xml"}, "exchange direction": "INPUT", "other": {"anies": [{"name": "referenceToUnitGroupDataSet", "value": {"shortDescription": [{"value": "MJ", "lang": "en"}], "type": "unit group data set", "refObjectId": "93a60a57-a3c8-11da-a746-0800200c9a66", "uri": "../unitgroups/93a60a57-a3c8-11da-a746-0800200c9a66.xml"}}, {"value": "49.884", "module": "A1-A3"}, {"value": "0.2311", "module": "A4"}, {"value": "1.77625", "module": "A5"}, {"value": "0", "module": "B1"}, {"value": "2.749", "module": "B2"}, {"value": "0", "module": "C1"}, {"value": "0.01286", "module": "C2"}, {"value": "0.6006", "module": "C3", "scenario": "S2"}, {"value": "0.8907", "module": "C3", "scenario": "S3"}, {"value": "0.4134", "module": "C4"}, {"value": "-0.1201", "module": "D", "scenario": "S0"}, {"value": "0", "module": "D", "scenario": "S1"}, {"value": "-1.689", "module": "D", "scenario": "S2"}, {"value": "-0.5789", "module": "D", "scenario": "S3"}]}, "resolvedFlowVersion": "38.00.000", "flowProperties": [], "typeOfFlow": "Other flow", "classification": {"classHierarchy": "Quantities", "name": "GaBiCategories"}}, {"dataSetInternalID": 2, "referenceToFlowDataSet": {"shortDescription": [{"value": "Renewable primary energy resources as material utilization (PERM)", "lang": "en"}, {"value": "Erneuerbare Primärenergie zur stofflichen Nutzung (PERM)", "lang": "de"}], "type": "flow data set", "refObjectId": "fb3ec0de-548d-4508-aea5-00b73bf6f702", "uri": "../flows/fb3ec0de-548d-4508-aea5-00b73bf6f702.xml"}, "exchange direction": "INPUT", "other": {"anies": [{"name": "referenceToUnitGroupDataSet", "value": {"shortDescription": [{"value": "MJ", "lang": "en"}], "type": "unit group data set", "refObjectId": "93a60a57-a3c8-11da-a746-0800200c9a66", "uri": "../unitgroups/93a60a57-a3c8-11da-a746-0800200c9a66.xml"}}, {"value": "0.246", "module": "A1-A3"}, {"value": "0", "module": "A4"}, {"value": "-0.246", "module": "A5"}, {"value": "0", "module": "B1"}, {"value": "0", "module": "B2"}, {"value": "0", "module": "C1"}, {"value": "0", "module": "C2"}, {"value": "0", "module": "C3", "scenario": "S2"}, {"value": "0", "module": "C3", "scenario": "S3"}, {"value": "0", "module": "C4"}, {"value": "0", "module": "D", "scenario": "S0"}, {"value": "0", "module": "D", "scenario": "S1"}, {"value": "0", "module": "D", "scenario": "S2"}, {"value": "0", "module": "D", "scenario": "S3"}]}, "resolvedFlowVersion": "38.00.000", "flowProperties": [], "typeOfFlow": "Other flow", "classification": {"classHierarchy": "Quantities", "name": "GaBiCategories"}}, {"dataSetInternalID": 3, "referenceToFlowDataSet": {"shortDescription": [{"value": "Total use of renewable primary energy resources (PERT)", "lang": "en"}, {"value": "Total erneuerbare Primärenergie (PERT)", "lang": "de"}], "type": "flow data set", "refObjectId": "53f97275-fa8a-4cdd-9024-65936002acd0", "uri": "../flows/53f97275-fa8a-4cdd-9024-65936002acd0.xml"}, "exchange direction": "INPUT", "other": {"anies": [{"name": "referenceToUnitGroupDataSet", "value": {"shortDescription": [{"value": "MJ", "lang": "en"}], "type": "unit group data set", "refObjectId": "93a60a57-a3c8-11da-a746-0800200c9a66", "uri": "../unitgroups/93a60a57-a3c8-11da-a746-0800200c9a66.xml"}}, {"value": "50.13", "module": "A1-A3"}, {"value": "0.2311", "module": "A4"}, {"value": "1.53025", "module": "A5"}, {"value": "0", "module": "B1"}, {"value": "2.749", "module": "B2"}, {"value": "0", "module": "C1"}, {"value": "0.01286", "module": "C2"}, {"value": "0.6006", "module": "C3", "scenario": "S2"}, {"value": "0.8907", "module": "C3", "scenario": "S3"}, {"value": "0.4134", "module": "C4"}, {"value": "-0.1201", "module": "D", "scenario": "S0"}, {"value": "0", "module": "D", "scenario": "S1"}, {"value": "-1.689", "module": "D", "scenario": "S2"}, {"value": "-0.5789", "module": "D", "scenario": "S3"}]}, "resolvedFlowVersion": "38.00.000", "flowProperties": [], "typeOfFlow": "Other flow", "classification": {"classHierarchy": "Quantities / Environmental quantities / EPD EN 15804 / LCI indicators", "name": "GaBiCategories"}}, {"dataSetInternalID": 4, "referenceToFlowDataSet": {"shortDescription": [{"value": "Non renewable primary energy as energy carrier (PENRE)", "lang": "en"}, {"value": "Nicht-erneuerbare Primärenergie als Energieträger (PENRE)", "lang": "de"}], "type": "flow data set", "refObjectId": "ac857178-2b45-46ec-892a-a9a4332f0372", "uri": "../flows/ac857178-2b45-46ec-892a-a9a4332f0372.xml"}, "exchange direction": "INPUT", "other": {"anies": [{"name": "referenceToUnitGroupDataSet", "value": {"shortDescription": [{"value": "MJ", "lang": "en"}], "type": "unit group data set", "refObjectId": "93a60a57-a3c8-11da-a746-0800200c9a66", "uri": "../unitgroups/93a60a57-a3c8-11da-a746-0800200c9a66.xml"}}, {"value": "88.308", "module": "A1-A3"}, {"value": "4.075", "module": "A4"}, {"value": "4.5001", "module": "A5"}, {"value": "0", "module": "B1"}, {"value": "4.502", "module": "B2"}, {"value": "0", "module": "C1"}, {"value": "0.2267", "module": "C2"}, {"value": "42.758", "module": "C3", "scenario": "S2"}, {"value": "43.79", "module": "C3", "scenario": "S3"}, {"value": "5.031", "module": "C4"}, {"value": "-0.4567", "module": "D", "scenario": "S0"}, {"value": "0", "module": "D", "scenario": "S1"}, {"value": "-6.848", "module": "D", "scenario": "S2"}, {"value": "-36.61", "module": "D", "scenario": "S3"}]}, "resolvedFlowVersion": "38.00.000", "flowProperties": [], "typeOfFlow": "Other flow", "classification": {"classHierarchy": "Quantities", "name": "GaBiCategories"}}, {"dataSetInternalID": 5, "referenceToFlowDataSet": {"shortDescription": [{"value": "Non renewable primary energy as material utilization (PENRM)", "lang": "en"}, {"value": "Nicht-erneuerbare Primärenergie zur stofflichen Nutzung (PENRM)", "lang": "de"}], "type": "flow data set", "refObjectId": "1421caa0-679d-4bf4-b282-0eb850ccae27", "uri": "../flows/1421caa0-679d-4bf4-b282-0eb850ccae27.xml"}, "exchange direction": "INPUT", "other": {"anies": [{"name": "referenceToUnitGroupDataSet", "value": {"shortDescription": [{"value": "MJ", "lang": "en"}], "type": "unit group data set", "refObjectId": "93a60a57-a3c8-11da-a746-0800200c9a66", "uri": "../unitgroups/93a60a57-a3c8-11da-a746-0800200c9a66.xml"}}, {"value": "39.692", "module": "A1-A3"}, {"value": "0", "module": "A4"}, {"value": "-0.42", "module": "A5"}, {"value": "0", "module": "B1"}, {"value": "0", "module": "B2"}, {"value": "0", "module": "C1"}, {"value": "0", "module": "C2"}, {"value": "-39.272", "module": "C3", "scenario": "S2"}, {"value": "-39.272", "module": "C3", "scenario": "S3"}, {"value": "0", "module": "C4"}, {"value": "0", "module": "D", "scenario": "S0"}, {"value": "0", "module": "D", "scenario": "S1"}, {"value": "0", "module": "D", "scenario": "S2"}, {"value": "0", "module": "D", "scenario": "S3"}]}, "resolvedFlowVersion": "38.00.000", "flowProperties": [], "typeOfFlow": "Other flow", "classification": {"classHierarchy": "Quantities", "name": "GaBiCategories"}}, {"dataSetInternalID": 6, "referenceToFlowDataSet": {"shortDescription": [{"value": "Total use of non renewable primary energy resources (PENRT)", "lang": "en"}, {"value": "Total nicht erneuerbare Primärenergie (PENRT)", "lang": "de"}], "type": "flow data set", "refObjectId": "06159210-646b-4c8d-8583-da9b3b95a6c1", "uri": "../flows/06159210-646b-4c8d-8583-da9b3b95a6c1.xml"}, "exchange direction": "INPUT", "other": {"anies": [{"name": "referenceToUnitGroupDataSet", "value": {"shortDescription": [{"value": "MJ", "lang": "en"}], "type": "unit group data set", "refObjectId": "93a60a57-a3c8-11da-a746-0800200c9a66", "uri": "../unitgroups/93a60a57-a3c8-11da-a746-0800200c9a66.xml"}}, {"value": "128", "module": "A1-A3"}, {"value": "4.075", "module": "A4"}, {"value": "4.0801", "module": "A5"}, {"value": "0", "module": "B1"}, {"value": "4.502", "module": "B2"}, {"value": "0", "module": "C1"}, {"value": "0.2267", "module": "C2"}, {"value": "3.486", "module": "C3", "scenario": "S2"}, {"value": "4.518", "module": "C3", "scenario": "S3"}, {"value": "5.031", "module": "C4"}, {"value": "-0.4567", "module": "D", "scenario": "S0"}, {"value": "0", "module": "D", "scenario": "S1"}, {"value": "-6.848", "module": "D", "scenario": "S2"}, {"value": "-36.61", "module": "D", "scenario": "S3"}]}, "resolvedFlowVersion": "38.00.000", "flowProperties": [], "typeOfFlow": "Other flow", "classification": {"classHierarchy": "Quantities / Environmental quantities / EPD EN 15804 / LCI indicators", "name": "GaBiCategories"}}, {"dataSetInternalID": 7, "referenceToFlowDataSet": {"shortDescription": [{"value": "Use of secondary material (SM)", "lang": "en"}, {"value": "Einsatz von Sekundärstoffen (SM)", "lang": "de"}], "type": "flow data set", "refObjectId": "c6a1f35f-2d09-4f54-8dfb-97e502e1ce92", "uri": "../flows/c6a1f35f-2d09-4f54-8dfb-97e502e1ce92.xml"}, "exchange direction": "INPUT", "other": {"anies": [{"name": "referenceToUnitGroupDataSet", "value": {"shortDescription": [{"value": "kg", "lang": "en"}], "type": "unit group data set", "refObjectId": "ad38d542-3fe9-439d-9b95-2f5f7752acaf", "uri": "../unitgroups/ad38d542-3fe9-439d-9b95-2f5f7752acaf.xml"}}, {"value": "1.036", "module": "A1-A3"}, {"value": "0", "module": "A4"}, {"value": "0.03108", "module": "A5"}, {"value": "0", "module": "B1"}, {"value": "0", "module": "B2"}, {"value": "0", "module": "C1"}, {"value": "0", "module": "C2"}, {"value": "0", "module": "C3", "scenario": "S2"}, {"value": "0", "module": "C3", "scenario": "S3"}, {"value": "0", "module": "C4"}, {"value": "0", "module": "D", "scenario": "S0"}, {"value": "0", "module": "D", "scenario": "S1"}, {"value": "0", "module": "D", "scenario": "S2"}, {"value": "1.7", "module": "D", "scenario": "S3"}]}, "resolvedFlowVersion": "38.00.000", "flowProperties": [], "typeOfFlow": "Other flow", "classification": {"classHierarchy": "Quantities / Environmental quantities / EPD EN 15804 / LCI indicators", "name": "GaBiCategories"}}, {"dataSetInternalID": 8, "referenceToFlowDataSet": {"shortDescription": [{"value": "Use of renewable secondary fuels (RSF)", "lang": "en"}, {"value": "Erneuerbare Sekundärbrennstoffe (RSF)", "lang": "de"}], "type": "flow data set", "refObjectId": "64333088-a55f-4aa2-9a31-c10b07816787", "uri": "../flows/64333088-a55f-4aa2-9a31-c10b07816787.xml"}, "exchange direction": "INPUT", "other": {"anies": [{"name": "referenceToUnitGroupDataSet", "value": {"shortDescription": [{"value": "MJ", "lang": "en"}], "type": "unit group data set", "refObjectId": "93a60a57-a3c8-11da-a746-0800200c9a66", "uri": "../unitgroups/93a60a57-a3c8-11da-a746-0800200c9a66.xml"}}, {"value": "0", "module": "A1-A3"}, {"value": "0", "module": "A4"}, {"value": "0", "module": "A5"}, {"value": "0", "module": "B1"}, {"value": "0", "module": "B2"}, {"value": "0", "module": "C1"}, {"value": "0", "module": "C2"}, {"value": "0", "module": "C3", "scenario": "S2"}, {"value": "0", "module": "C3", "scenario": "S3"}, {"value": "0", "module": "C4"}, {"value": "0", "module": "D", "scenario": "S0"}, {"value": "0", "module": "D", "scenario": "S1"}, {"value": "0", "module": "D", "scenario": "S2"}, {"value": "0", "module": "D", "scenario": "S3"}]}, "resolvedFlowVersion": "38.00.000", "flowProperties": [], "typeOfFlow": "Other flow", "classification": {"classHierarchy": "Quantities / Environmental quantities / EPD EN 15804 / LCI indicators", "name": "GaBiCategories"}}, {"dataSetInternalID": 9, "referenceToFlowDataSet": {"shortDescription": [{"value": "Use of non renewable secondary fuels (NRSF)", "lang": "en"}, {"value": "Nicht erneuerbare Sekundärbrennstoffe (NRSF)", "lang": "de"}], "type": "flow data set", "refObjectId": "89def144-d39a-4287-b86f-efde453ddcb2", "uri": "../flows/89def144-d39a-4287-b86f-efde453ddcb2.xml"}, "exchange direction": "INPUT", "other": {"anies": [{"name": "referenceToUnitGroupDataSet", "value": {"shortDescription": [{"value": "MJ", "lang": "en"}], "type": "unit group data set", "refObjectId": "93a60a57-a3c8-11da-a746-0800200c9a66", "uri": "../unitgroups/93a60a57-a3c8-11da-a746-0800200c9a66.xml"}}, {"value": "0", "module": "A1-A3"}, {"value": "0", "module": "A4"}, {"value": "0", "module": "A5"}, {"value": "0", "module": "B1"}, {"value": "0", "module": "B2"}, {"value": "0", "module": "C1"}, {"value": "0", "module": "C2"}, {"value": "0", "module": "C3", "scenario": "S2"}, {"value": "0", "module": "C3", "scenario": "S3"}, {"value": "0", "module": "C4"}, {"value": "0", "module": "D", "scenario": "S0"}, {"value": "0", "module": "D", "scenario": "S1"}, {"value": "0", "module": "D", "scenario": "S2"}, {"value": "0", "module": "D", "scenario": "S3"}]}, "resolvedFlowVersion": "38.00.000", "flowProperties": [], "typeOfFlow": "Other flow", "classification": {"classHierarchy": "Quantities / Environmental quantities / EPD EN 15804 / LCI indicators", "name": "GaBiCategories"}}, {"dataSetInternalID": 10, "referenceToFlowDataSet": {"shortDescription": [{"value": "Use of net fresh water (FW)", "lang": "en"}, {"value": "Einsatz von Süßwasserressourcen (FW)", "lang": "de"}], "type": "flow data set", "refObjectId": "3cf952c8-f3a4-461d-8c96-96456ca62246", "uri": "../flows/3cf952c8-f3a4-461d-8c96-96456ca62246.xml"}, "exchange direction": "INPUT", "other": {"anies": [{"name": "referenceToUnitGroupDataSet", "value": {"shortDescription": [{"value": "m^3", "lang": "en"}], "type": "unit group data set", "refObjectId": "cd950537-0a98-4044-9ba7-9f9a68d0a504", "uri": "../unitgroups/cd950537-0a98-4044-9ba7-9f9a68d0a504.xml"}}, {"value": "0.1257", "module": "A1-A3"}, {"value": "0.0002612", "module": "A4"}, {"value": "0.0043864", "module": "A5"}, {"value": "0", "module": "B1"}, {"value": "0.002518", "module": "B2"}, {"value": "0", "module": "C1"}, {"value": "1.453E-05", "module": "C2"}, {"value": "0.01798", "module": "C3", "scenario": "S2"}, {"value": "0.01826", "module": "C3", "scenario": "S3"}, {"value": "5.889E-05", "module": "C4"}, {"value": "-0.0001148", "module": "D", "scenario": "S0"}, {"value": "0", "module": "D", "scenario": "S1"}, {"value": "-0.001615", "module": "D", "scenario": "S2"}, {"value": "-0.003537", "module": "D", "scenario": "S3"}]}, "resolvedFlowVersion": "38.00.000", "flowProperties": [], "typeOfFlow": "Other flow", "classification": {"classHierarchy": "Quantities / Environmental quantities / EPD EN 15804 / LCI indicators", "name": "GaBiCategories"}}, {"dataSetInternalID": 11, "referenceToFlowDataSet": {"shortDescription": [{"value": "Hazardous waste disposed (HWD)", "lang": "en"}, {"value": "Gefährlicher Abfall zur Deponie (HWD)", "lang": "de"}], "type": "flow data set", "refObjectId": "430f9e0f-59b2-46a0-8e0d-55e0e84948fc", "uri": "../flows/430f9e0f-59b2-46a0-8e0d-55e0e84948fc.xml"}, "exchange direction": "OUTPUT", "other": {"anies": [{"name": "referenceToUnitGroupDataSet", "value": {"shortDescription": [{"value": "kg", "lang": "en"}], "type": "unit group data set", "refObjectId": "ad38d542-3fe9-439d-9b95-2f5f7752acaf", "uri": "../unitgroups/ad38d542-3fe9-439d-9b95-2f5f7752acaf.xml"}}, {"value": "0.00255", "module": "A1-A3"}, {"value": "1.95E-11", "module": "A4"}, {"value": "7.65000165E-05", "module": "A5"}, {"value": "0", "module": "B1"}, {"value": "2.56E-05", "module": "B2"}, {"value": "0", "module": "C1"}, {"value": "1.09E-12", "module": "C2"}, {"value": "5.18E-10", "module": "C3", "scenario": "S2"}, {"value": "5.61E-10", "module": "C3", "scenario": "S3"}, {"value": "7.76E-10", "module": "C4"}, {"value": "-6.28E-11", "module": "D", "scenario": "S0"}, {"value": "0", "module": "D", "scenario": "S1"}, {"value": "-9.6E-10", "module": "D", "scenario": "S2"}, {"value": "-3.36E-10", "module": "D", "scenario": "S3"}]}, "resolvedFlowVersion": "38.00.000", "flowProperties": [], "typeOfFlow": "Other flow", "classification": {"classHierarchy": "Quantities / Environmental quantities / EPD EN 15804 / LCI indicators", "name": "GaBiCategories"}}, {"dataSetInternalID": 12, "referenceToFlowDataSet": {"shortDescription": [{"value": "Non hazardous waste disposed (NHWD)", "lang": "en"}, {"value": "Entsorgter nicht gefährlicher Abfall (NHWD)", "lang": "de"}], "type": "flow data set", "refObjectId": "b29ef66b-e286-4afa-949f-62f1a7b4d7fa", "uri": "../flows/b29ef66b-e286-4afa-949f-62f1a7b4d7fa.xml"}, "exchange direction": "OUTPUT", "other": {"anies": [{"name": "referenceToUnitGroupDataSet", "value": {"shortDescription": [{"value": "kg", "lang": "en"}], "type": "unit group data set", "refObjectId": "ad38d542-3fe9-439d-9b95-2f5f7752acaf", "uri": "../unitgroups/ad38d542-3fe9-439d-9b95-2f5f7752acaf.xml"}}, {"value": "0.719", "module": "A1-A3"}, {"value": "0.000584", "module": "A4"}, {"value": "0.06707", "module": "A5"}, {"value": "0", "module": "B1"}, {"value": "0.00514", "module": "B2"}, {"value": "0", "module": "C1"}, {"value": "3.25E-05", "module": "C2"}, {"value": "1.51", "module": "C3", "scenario": "S2"}, {"value": "1.51", "module": "C3", "scenario": "S3"}, {"value": "4.98", "module": "C4"}, {"value": "-0.000226", "module": "D", "scenario": "S0"}, {"value": "0", "module": "D", "scenario": "S1"}, {"value": "-0.00329", "module": "D", "scenario": "S2"}, {"value": "-0.204", "module": "D", "scenario": "S3"}]}, "resolvedFlowVersion": "38.00.000", "flowProperties": [], "typeOfFlow": "Other flow", "classification": {"classHierarchy": "Quantities / Environmental quantities / EPD EN 15804 / LCI indicators", "name": "GaBiCategories"}}, {"dataSetInternalID": 13, "referenceToFlowDataSet": {"shortDescription": [{"value": "Radioactive waste disposed (RWD)", "lang": "en"}, {"value": "Entsorgter radioaktiver Abfall (RWD)", "lang": "de"}], "type": "flow data set", "refObjectId": "3449546e-52ad-4b39-b809-9fb77cea8ff6", "uri": "../flows/3449546e-52ad-4b39-b809-9fb77cea8ff6.xml"}, "exchange direction": "OUTPUT", "other": {"anies": [{"name": "referenceToUnitGroupDataSet", "value": {"shortDescription": [{"value": "kg", "lang": "en"}], "type": "unit group data set", "refObjectId": "ad38d542-3fe9-439d-9b95-2f5f7752acaf", "uri": "../unitgroups/ad38d542-3fe9-439d-9b95-2f5f7752acaf.xml"}}, {"value": "0.00279", "module": "A1-A3"}, {"value": "5.02E-06", "module": "A4"}, {"value": "8.798E-05", "module": "A5"}, {"value": "0", "module": "B1"}, {"value": "0.000374", "module": "B2"}, {"value": "0", "module": "C1"}, {"value": "2.79E-07", "module": "C2"}, {"value": "0.00013", "module": "C3", "scenario": "S2"}, {"value": "0.000205", "module": "C3", "scenario": "S3"}, {"value": "6.18E-05", "module": "C4"}, {"value": "-3.44E-05", "module": "D", "scenario": "S0"}, {"value": "0", "module": "D", "scenario": "S1"}, {"value": "-0.000484", "module": "D", "scenario": "S2"}, {"value": "-0.000122", "module": "D", "scenario": "S3"}]}, "resolvedFlowVersion": "38.00.000", "flowProperties": [], "typeOfFlow": "Other flow", "classification": {"classHierarchy": "Quantities / Environmental quantities / EPD EN 15804 / LCI indicators", "name": "GaBiCategories"}}, {"dataSetInternalID": 14, "referenceToFlowDataSet": {"shortDescription": [{"value": "Components for re-use (CRU)", "lang": "en"}, {"value": "Komponenten für die Wiederverwendung (CRU)", "lang": "de"}], "type": "flow data set", "refObjectId": "a2b32f97-3fc7-4af2-b209-525bc6426f33", "uri": "../flows/a2b32f97-3fc7-4af2-b209-525bc6426f33.xml"}, "exchange direction": "OUTPUT", "other": {"anies": [{"name": "referenceToUnitGroupDataSet", "value": {"shortDescription": [{"value": "kg", "lang": "en"}], "type": "unit group data set", "refObjectId": "ad38d542-3fe9-439d-9b95-2f5f7752acaf", "uri": "../unitgroups/ad38d542-3fe9-439d-9b95-2f5f7752acaf.xml"}}, {"value": "0", "module": "A1-A3"}, {"value": "0", "module": "A4"}, {"value": "0", "module": "A5"}, {"value": "0", "module": "B1"}, {"value": "0", "module": "B2"}, {"value": "0", "module": "C1"}, {"value": "0", "module": "C2"}, {"value": "0", "module": "C3", "scenario": "S2"}, {"value": "0", "module": "C3", "scenario": "S3"}, {"value": "0", "module": "C4"}, {"value": "0", "module": "D", "scenario": "S0"}, {"value": "0", "module": "D", "scenario": "S1"}, {"value": "0", "module": "D", "scenario": "S2"}, {"value": "0", "module": "D", "scenario": "S3"}]}, "resolvedFlowVersion": "38.00.000", "flowProperties": [], "typeOfFlow": "Other flow", "classification": {"classHierarchy": "Quantities / Environmental quantities / EPD EN 15804 / LCI indicators", "name": "GaBiCategories"}}, {"dataSetInternalID": 15, "referenceToFlowDataSet": {"shortDescription": [{"value": "Materials for recycling (MFR)", "lang": "en"}, {"value": "Stoffe zum Recycling (MFR)", "lang": "de"}], "type": "flow data set", "refObjectId": "d7fe48a5-4103-49c8-9aae-b0b5dfdbd6ae", "uri": "../flows/d7fe48a5-4103-49c8-9aae-b0b5dfdbd6ae.xml"}, "exchange direction": "OUTPUT", "other": {"anies": [{"name": "referenceToUnitGroupDataSet", "value": {"shortDescription": [{"value": "kg", "lang": "en"}], "type": "unit group data set", "refObjectId": "ad38d542-3fe9-439d-9b95-2f5f7752acaf", "uri": "../unitgroups/ad38d542-3fe9-439d-9b95-2f5f7752acaf.xml"}}, {"value": "0.0171", "module": "A1-A3"}, {"value": "0", "module": "A4"}, {"value": "0.126513", "module": "A5"}, {"value": "0", "module": "B1"}, {"value": "0", "module": "B2"}, {"value": "0", "module": "C1"}, {"value": "0", "module": "C2"}, {"value": "0", "module": "C3", "scenario": "S2"}, {"value": "1.7", "module": "C3", "scenario": "S3"}, {"value": "0", "module": "C4"}, {"value": "0", "module": "D", "scenario": "S0"}, {"value": "0", "module": "D", "scenario": "S1"}, {"value": "0", "module": "D", "scenario": "S2"}, {"value": "0", "module": "D", "scenario": "S3"}]}, "resolvedFlowVersion": "38.00.000", "flowProperties": [], "typeOfFlow": "Other flow", "classification": {"classHierarchy": "Quantities / Environmental quantities / EPD EN 15804 / LCI indicators", "name": "GaBiCategories"}}, {"dataSetInternalID": 16, "referenceToFlowDataSet": {"shortDescription": [{"value": "Materials for energy recovery (MER)", "lang": "en"}, {"value": "Stoffe für die Energierückgewinnung (MER)", "lang": "de"}], "type": "flow data set", "refObjectId": "59a9181c-3aaf-46ee-8b13-2b3723b6e447", "uri": "../flows/59a9181c-3aaf-46ee-8b13-2b3723b6e447.xml"}, "exchange direction": "OUTPUT", "other": {"anies": [{"name": "referenceToUnitGroupDataSet", "value": {"shortDescription": [{"value": "kg", "lang": "en"}], "type": "unit group data set", "refObjectId": "ad38d542-3fe9-439d-9b95-2f5f7752acaf", "uri": "../unitgroups/ad38d542-3fe9-439d-9b95-2f5f7752acaf.xml"}}, {"value": "0", "module": "A1-A3"}, {"value": "0", "module": "A4"}, {"value": "0", "module": "A5"}, {"value": "0", "module": "B1"}, {"value": "0", "module": "B2"}, {"value": "0", "module": "C1"}, {"value": "0", "module": "C2"}, {"value": "0", "module": "C3", "scenario": "S2"}, {"value": "0", "module": "C3", "scenario": "S3"}, {"value": "0", "module": "C4"}, {"value": "0", "module": "D", "scenario": "S0"}, {"value": "0", "module": "D", "scenario": "S1"}, {"value": "0", "module": "D", "scenario": "S2"}, {"value": "0", "module": "D", "scenario": "S3"}]}, "resolvedFlowVersion": "38.00.000", "flowProperties": [], "typeOfFlow": "Other flow", "classification": {"classHierarchy": "Quantities / Environmental quantities / EPD EN 15804 / LCI indicators", "name": "GaBiCategories"}}, {"dataSetInternalID": 17, "referenceToFlowDataSet": {"shortDescription": [{"value": "Exported electrical energy (EEE)", "lang": "en"}, {"value": "Exportierte elektrische Energie (EEE)", "lang": "de"}], "type": "flow data set", "refObjectId": "4da0c987-2b76-40d6-9e9e-82a017aaaf29", "uri": "../flows/4da0c987-2b76-40d6-9e9e-82a017aaaf29.xml"}, "exchange direction": "OUTPUT", "other": {"anies": [{"name": "referenceToUnitGroupDataSet", "value": {"shortDescription": [{"value": "MJ", "lang": "en"}], "type": "unit group data set", "refObjectId": "93a60a57-a3c8-11da-a746-0800200c9a66", "uri": "../unitgroups/93a60a57-a3c8-11da-a746-0800200c9a66.xml"}}, {"value": "0", "module": "A1-A3"}, {"value": "0", "module": "A4"}, {"value": "0.235", "module": "A5"}, {"value": "0", "module": "B1"}, {"value": "0", "module": "B2"}, {"value": "0", "module": "C1"}, {"value": "0", "module": "C2"}, {"value": "5.62", "module": "C3", "scenario": "S2"}, {"value": "0", "module": "C3", "scenario": "S3"}, {"value": "0", "module": "C4"}, {"value": "0", "module": "D", "scenario": "S0"}, {"value": "0", "module": "D", "scenario": "S1"}, {"value": "0", "module": "D", "scenario": "S2"}, {"value": "0", "module": "D", "scenario": "S3"}]}, "resolvedFlowVersion": "38.00.000", "flowProperties": [], "typeOfFlow": "Other flow", "classification": {"classHierarchy": "Quantities / Environmental quantities / EPD EN 15804 / LCI indicators", "name": "GaBiCategories"}}, {"dataSetInternalID": 18, "referenceToFlowDataSet": {"shortDescription": [{"value": "Exported thermal energy (EET)", "lang": "en"}, {"value": "Exportierte thermische Energie (EET)", "lang": "de"}], "type": "flow data set", "refObjectId": "98daf38a-7a79-46d3-9a37-2b7bd0955810", "uri": "../flows/98daf38a-7a79-46d3-9a37-2b7bd0955810.xml"}, "exchange direction": "OUTPUT", "other": {"anies": [{"name": "referenceToUnitGroupDataSet", "value": {"shortDescription": [{"value": "MJ", "lang": "en"}], "type": "unit group data set", "refObjectId": "93a60a57-a3c8-11da-a746-0800200c9a66", "uri": "../unitgroups/93a60a57-a3c8-11da-a746-0800200c9a66.xml"}}, {"value": "0", "module": "A1-A3"}, {"value": "0", "module": "A4"}, {"value": "0.44", "module": "A5"}, {"value": "0", "module": "B1"}, {"value": "0", "module": "B2"}, {"value": "0", "module": "C1"}, {"value": "0", "module": "C2"}, {"value": "10.7", "module": "C3", "scenario": "S2"}, {"value": "66.5", "module": "C3", "scenario": "S3"}, {"value": "0", "module": "C4"}, {"value": "0", "module": "D", "scenario": "S0"}, {"value": "0", "module": "D", "scenario": "S1"}, {"value": "0", "module": "D", "scenario": "S2"}, {"value": "0", "module": "D", "scenario": "S3"}]}, "resolvedFlowVersion": "38.00.000", "flowProperties": [], "typeOfFlow": "Other flow", "classification": {"classHierarchy": "Quantities / Environmental quantities / EPD EN 15804 / LCI indicators", "name": "GaBiCategories"}}]}, "LCIAResults": {"LCIAResult": [{"referenceToLCIAMethodDataSet": {"shortDescription": [{"value": "Global Warming Potential total (GWP-total)", "lang": "en"}, {"value": "Globales Erwärmungspotenzial total (GWP-total)", "lang": "de"}], "type": "LCIA method data set", "refObjectId": "6a37f984-a4b3-458a-a20a-64418c145fa2", "uri": "../lciamethods/6a37f984-a4b3-458a-a20a-64418c145fa2.xml"}, "other": {"anies": [{"name": "referenceToUnitGroupDataSet", "value": {"shortDescription": [{"value": "kg CO_(2) eq", "lang": "en"}], "type": "unit group data set", "refObjectId": "1ebf3012-d0db-4de2-aefd-ef30cedb0be1", "uri": "../unitgroups/1ebf3012-d0db-4de2-aefd-ef30cedb0be1.xml"}}, {"value": "5.854", "module": "A1-A3"}, {"value": "0.3051", "module": "A4"}, {"value": "0.57022", "module": "A5"}, {"value": "0", "module": "B1"}, {"value": "0.385", "module": "B2"}, {"value": "0", "module": "C1"}, {"value": "0.01697", "module": "C2"}, {"value": "5.046", "module": "C3", "scenario": "S2"}, {"value": "5.115", "module": "C3", "scenario": "S3"}, {"value": "0.3508", "module": "C4"}, {"value": "-0.02706", "module": "D", "scenario": "S0"}, {"value": "0", "module": "D", "scenario": "S1"}, {"value": "-0.4071", "module": "D", "scenario": "S2"}, {"value": "-0.36", "module": "D", "scenario": "S3"}]}}, {"referenceToLCIAMethodDataSet": {"shortDescription": [{"value": "Global Warming Potential fossil fuels (GWP-fossil)", "lang": "en"}, {"value": "Globales Erwärmungspotenzial fossil (GWP-fossil)", "lang": "de"}], "type": "LCIA method data set", "refObjectId": "5f635281-343e-44fb-83df-1971b155e6b6", "uri": "../lciamethods/5f635281-343e-44fb-83df-1971b155e6b6.xml"}, "other": {"anies": [{"name": "referenceToUnitGroupDataSet", "value": {"shortDescription": [{"value": "kg CO_(2) eq", "lang": "en"}], "type": "unit group data set", "refObjectId": "1ebf3012-d0db-4de2-aefd-ef30cedb0be1", "uri": "../unitgroups/1ebf3012-d0db-4de2-aefd-ef30cedb0be1.xml"}}, {"value": "6.041", "module": "A1-A3"}, {"value": "0.2995", "module": "A4"}, {"value": "0.37363", "module": "A5"}, {"value": "0", "module": "B1"}, {"value": "0.2623", "module": "B2"}, {"value": "0", "module": "C1"}, {"value": "0.01666", "module": "C2"}, {"value": "5.045", "module": "C3", "scenario": "S2"}, {"value": "5.112", "module": "C3", "scenario": "S3"}, {"value": "0.3506", "module": "C4"}, {"value": "-0.02692", "module": "D", "scenario": "S0"}, {"value": "0", "module": "D", "scenario": "S1"}, {"value": "-0.4051", "module": "D", "scenario": "S2"}, {"value": "-0.3596", "module": "D", "scenario": "S3"}]}}, {"referenceToLCIAMethodDataSet": {"shortDescription": [{"value": "Global Warming Potential biogenic (GWP-biogenic)", "lang": "en"}, {"value": "Globales Erwärmungspotenzial biogen (GWP-biogenic)", "lang": "de"}], "type": "LCIA method data set", "refObjectId": "2356e1ab-0185-4db5-86e5-16de51c7485c", "uri": "../lciamethods/2356e1ab-0185-4db5-86e5-16de51c7485c.xml"}, "other": {"anies": [{"name": "referenceToUnitGroupDataSet", "value": {"shortDescription": [{"value": "kg CO_(2) eq", "lang": "en"}], "type": "unit group data set", "refObjectId": "1ebf3012-d0db-4de2-aefd-ef30cedb0be1", "uri": "../unitgroups/1ebf3012-d0db-4de2-aefd-ef30cedb0be1.xml"}}, {"value": "-0.1927", "module": "A1-A3"}, {"value": "0.003876", "module": "A4"}, {"value": "0.196319", "module": "A5"}, {"value": "0", "module": "B1"}, {"value": "0.002986", "module": "B2"}, {"value": "0", "module": "C1"}, {"value": "0.0002156", "module": "C2"}, {"value": "0.0007687", "module": "C3", "scenario": "S2"}, {"value": "0.001538", "module": "C3", "scenario": "S3"}, {"value": "-5.76E-08", "module": "C4"}, {"value": "-0.0001336", "module": "D", "scenario": "S0"}, {"value": "0", "module": "D", "scenario": "S1"}, {"value": "-0.001926", "module": "D", "scenario": "S2"}, {"value": "-0.000283", "module": "D", "scenario": "S3"}]}}, {"referenceToLCIAMethodDataSet": {"shortDescription": [{"value": "Global Warming Potential luluc (GWP-luluc)", "lang": "en"}, {"value": "Globales Erwärmungspotenzial luluc (GWP-luluc)", "lang": "de"}], "type": "LCIA method data set", "refObjectId": "4331bbdb-978a-490d-8707-eeb047f01a55", "uri": "../lciamethods/4331bbdb-978a-490d-8707-eeb047f01a55.xml"}, "other": {"anies": [{"name": "referenceToUnitGroupDataSet", "value": {"shortDescription": [{"value": "kg CO_(2) eq", "lang": "en"}], "type": "unit group data set", "refObjectId": "1ebf3012-d0db-4de2-aefd-ef30cedb0be1", "uri": "../unitgroups/1ebf3012-d0db-4de2-aefd-ef30cedb0be1.xml"}}, {"value": "0.006163", "module": "A1-A3"}, {"value": "0.001696", "module": "A4"}, {"value": "0.00024894", "module": "A5"}, {"value": "0", "module": "B1"}, {"value": "0.1197", "module": "B2"}, {"value": "0", "module": "C1"}, {"value": "9.435E-05", "module": "C2"}, {"value": "0.0003052", "module": "C3", "scenario": "S2"}, {"value": "0.0005465", "module": "C3", "scenario": "S3"}, {"value": "0.0001725", "module": "C4"}, {"value": "-2.852E-06", "module": "D", "scenario": "S0"}, {"value": "0", "module": "D", "scenario": "S1"}, {"value": "-4.071E-05", "module": "D", "scenario": "S2"}, {"value": "-0.0001993", "module": "D", "scenario": "S3"}]}}, {"referenceToLCIAMethodDataSet": {"shortDescription": [{"value": "Depletion potential of the stratospheric ozone layer (ODP)", "lang": "en"}, {"value": "Abbau Potential der stratosphärischen Ozonschicht (ODP)", "lang": "de"}], "type": "LCIA method data set", "refObjectId": "b5c629d6-def3-11e6-bf01-fe55135034f3", "uri": "../lciamethods/b5c629d6-def3-11e6-bf01-fe55135034f3.xml"}, "other": {"anies": [{"name": "referenceToUnitGroupDataSet", "value": {"shortDescription": [{"value": "kg CFC11 eq", "lang": "en"}], "type": "unit group data set", "refObjectId": "d9e957c9-7309-4474-bf3a-7777df6c4e5b", "uri": "../unitgroups/d9e957c9-7309-4474-bf3a-7777df6c4e5b.xml"}}, {"value": "1.02E-08", "module": "A1-A3"}, {"value": "1.823E-14", "module": "A4"}, {"value": "3.0601482E-10", "module": "A5"}, {"value": "0", "module": "B1"}, {"value": "2.083E-08", "module": "B2"}, {"value": "0", "module": "C1"}, {"value": "1.014E-15", "module": "C2"}, {"value": "4.295E-13", "module": "C3", "scenario": "S2"}, {"value": "8.07E-13", "module": "C3", "scenario": "S3"}, {"value": "4.76E-13", "module": "C4"}, {"value": "-1.737E-13", "module": "D", "scenario": "S0"}, {"value": "0", "module": "D", "scenario": "S1"}, {"value": "-2.443E-12", "module": "D", "scenario": "S2"}, {"value": "-4.948E-13", "module": "D", "scenario": "S3"}]}}, {"referenceToLCIAMethodDataSet": {"shortDescription": [{"value": "Acidification potential of land and water (AP)", "lang": "en"}, {"value": "Versauerungspotenzial von Boden und Wasser (AP)", "lang": "de"}], "type": "LCIA method data set", "refObjectId": "b5c611c6-def3-11e6-bf01-fe55135034f3", "uri": "../lciamethods/b5c611c6-def3-11e6-bf01-fe55135034f3.xml"}, "other": {"anies": [{"name": "referenceToUnitGroupDataSet", "value": {"shortDescription": [{"value": "mol H^(+) eq", "lang": "en"}], "type": "unit group data set", "refObjectId": "42e089ac-92bf-4bf2-8ca1-5fc40d18f2ed", "uri": "../unitgroups/42e089ac-92bf-4bf2-8ca1-5fc40d18f2ed.xml"}}, {"value": "0.01718", "module": "A1-A3"}, {"value": "0.001811", "module": "A4"}, {"value": "0.0007184", "module": "A5"}, {"value": "0", "module": "B1"}, {"value": "0.0006168", "module": "B2"}, {"value": "0", "module": "C1"}, {"value": "0.0001007", "module": "C2"}, {"value": "0.004709", "module": "C3", "scenario": "S2"}, {"value": "0.005017", "module": "C3", "scenario": "S3"}, {"value": "0.00105", "module": "C4"}, {"value": "-3.449E-05", "module": "D", "scenario": "S0"}, {"value": "0", "module": "D", "scenario": "S1"}, {"value": "-0.0004998", "module": "D", "scenario": "S2"}, {"value": "-0.001457", "module": "D", "scenario": "S3"}]}}, {"referenceToLCIAMethodDataSet": {"shortDescription": [{"value": "Eutrophication potential aquatic freshwater (EP-freshwater)", "lang": "en"}, {"value": "Eutrophierungspotenzial Süßwasser (EP-freshwater)", "lang": "de"}], "type": "LCIA method data set", "refObjectId": "b53ec18f-7377-4ad3-86eb-cc3f4f276b2b", "uri": "../lciamethods/b53ec18f-7377-4ad3-86eb-cc3f4f276b2b.xml"}, "other": {"anies": [{"name": "referenceToUnitGroupDataSet", "value": {"shortDescription": [{"value": "kg P eq", "lang": "en"}], "type": "unit group data set", "refObjectId": "0429039d-a61d-4590-ba67-aa4a20a810a1", "uri": "../unitgroups/0429039d-a61d-4590-ba67-aa4a20a810a1.xml"}}, {"value": "5.637E-05", "module": "A1-A3"}, {"value": "9.081E-07", "module": "A4"}, {"value": "1.75267E-06", "module": "A5"}, {"value": "0", "module": "B1"}, {"value": "3.311E-06", "module": "B2"}, {"value": "0", "module": "C1"}, {"value": "5.051E-08", "module": "C2"}, {"value": "1.063E-06", "module": "C3", "scenario": "S2"}, {"value": "1.264E-06", "module": "C3", "scenario": "S3"}, {"value": "6.615E-05", "module": "C4"}, {"value": "-3.542E-08", "module": "D", "scenario": "S0"}, {"value": "0", "module": "D", "scenario": "S1"}, {"value": "-4.994E-07", "module": "D", "scenario": "S2"}, {"value": "-4.762E-07", "module": "D", "scenario": "S3"}]}}, {"referenceToLCIAMethodDataSet": {"shortDescription": [{"value": "Eutrophication potential aquatic marine (EP-marine)", "lang": "en"}, {"value": "Eutrophierungspotenzial Salzwasser (EP-marine)", "lang": "de"}], "type": "LCIA method data set", "refObjectId": "b5c619fa-def3-11e6-bf01-fe55135034f3", "uri": "../lciamethods/b5c619fa-def3-11e6-bf01-fe55135034f3.xml"}, "other": {"anies": [{"name": "referenceToUnitGroupDataSet", "value": {"shortDescription": [{"value": "kg N eq", "lang": "en"}], "type": "unit group data set", "refObjectId": "d05bb823-ecdf-4686-8c40-bf1d9257859f", "uri": "../unitgroups/d05bb823-ecdf-4686-8c40-bf1d9257859f.xml"}}, {"value": "0.005752", "module": "A1-A3"}, {"value": "0.0008891", "module": "A4"}, {"value": "0.00026986", "module": "A5"}, {"value": "0", "module": "B1"}, {"value": "0.0001447", "module": "B2"}, {"value": "0", "module": "C1"}, {"value": "4.946E-05", "module": "C2"}, {"value": "0.002263", "module": "C3", "scenario": "S2"}, {"value": "0.002399", "module": "C3", "scenario": "S3"}, {"value": "0.0002324", "module": "C4"}, {"value": "-9.465E-06", "module": "D", "scenario": "S0"}, {"value": "0", "module": "D", "scenario": "S1"}, {"value": "-0.0001395", "module": "D", "scenario": "S2"}, {"value": "-0.000437", "module": "D", "scenario": "S3"}]}}, {"referenceToLCIAMethodDataSet": {"shortDescription": [{"value": "Eutrophication potential terrestrial (EP-terrestrial)", "lang": "en"}, {"value": "Eutrophierungspotenzial Land (EP-terrestrial)", "lang": "de"}], "type": "LCIA method data set", "refObjectId": "b5c614d2-def3-11e6-bf01-fe55135034f3", "uri": "../lciamethods/b5c614d2-def3-11e6-bf01-fe55135034f3.xml"}, "other": {"anies": [{"name": "referenceToUnitGroupDataSet", "value": {"shortDescription": [{"value": "mol N eq", "lang": "en"}], "type": "unit group data set", "refObjectId": "71b4d617-0ec9-4d3f-b65e-e438940c2401", "uri": "../unitgroups/71b4d617-0ec9-4d3f-b65e-e438940c2401.xml"}}, {"value": "0.05413", "module": "A1-A3"}, {"value": "0.009842", "module": "A4"}, {"value": "0.0027129", "module": "A5"}, {"value": "0", "module": "B1"}, {"value": "0.001984", "module": "B2"}, {"value": "0", "module": "C1"}, {"value": "0.0005475", "module": "C2"}, {"value": "0.02519", "module": "C3", "scenario": "S2"}, {"value": "0.02669", "module": "C3", "scenario": "S3"}, {"value": "0.002548", "module": "C4"}, {"value": "-0.0001015", "module": "D", "scenario": "S0"}, {"value": "0", "module": "D", "scenario": "S1"}, {"value": "-0.001498", "module": "D", "scenario": "S2"}, {"value": "-0.004791", "module": "D", "scenario": "S3"}]}}, {"referenceToLCIAMethodDataSet": {"shortDescription": [{"value": "Formation potential of tropospheric ozone photochemical oxidants (POCP)", "lang": "en"}, {"value": "Bildungspotential für troposphärisches Ozon (POCP)", "lang": "de"}], "type": "LCIA method data set", "refObjectId": "b5c610fe-def3-11e6-bf01-fe55135034f3", "uri": "../lciamethods/b5c610fe-def3-11e6-bf01-fe55135034f3.xml"}, "other": {"anies": [{"name": "referenceToUnitGroupDataSet", "value": {"shortDescription": [{"value": "kg NMVOC eq", "lang": "en"}], "type": "unit group data set", "refObjectId": "d27c25f8-fbc1-44c6-b47b-4adbae4199c6", "uri": "../unitgroups/d27c25f8-fbc1-44c6-b47b-4adbae4199c6.xml"}}, {"value": "0.01536", "module": "A1-A3"}, {"value": "0.001681", "module": "A4"}, {"value": "0.0006916", "module": "A5"}, {"value": "0.000418", "module": "B1"}, {"value": "0.0006661", "module": "B2"}, {"value": "0", "module": "C1"}, {"value": "9.351E-05", "module": "C2"}, {"value": "0.005816", "module": "C3", "scenario": "S2"}, {"value": "0.006084", "module": "C3", "scenario": "S3"}, {"value": "0.0007475", "module": "C4"}, {"value": "-2.654E-05", "module": "D", "scenario": "S0"}, {"value": "0", "module": "D", "scenario": "S1"}, {"value": "-0.0003921", "module": "D", "scenario": "S2"}, {"value": "-0.001285", "module": "D", "scenario": "S3"}]}}, {"referenceToLCIAMethodDataSet": {"shortDescription": [{"value": "Abiotic depletion potential for non fossil resources (ADPE)", "lang": "en"}, {"value": "Potenzial für den abiotischen Abbau nicht fossiler Ressourcen (ADPE)", "lang": "de"}], "type": "LCIA method data set", "refObjectId": "b2ad6494-c78d-11e6-9d9d-cec0c932ce01", "uri": "../lciamethods/b2ad6494-c78d-11e6-9d9d-cec0c932ce01.xml"}, "other": {"anies": [{"name": "referenceToUnitGroupDataSet", "value": {"shortDescription": [{"value": "kg Sb eq", "lang": "en"}], "type": "unit group data set", "refObjectId": "54ccd2d9-a32a-4fc2-923d-f2c8c93e89d4", "uri": "../unitgroups/54ccd2d9-a32a-4fc2-923d-f2c8c93e89d4.xml"}}, {"value": "1.694E-06", "module": "A1-A3"}, {"value": "2.543E-08", "module": "A4"}, {"value": "5.2584E-08", "module": "A5"}, {"value": "0", "module": "B1"}, {"value": "1.539E-07", "module": "B2"}, {"value": "0", "module": "C1"}, {"value": "1.415E-09", "module": "C2"}, {"value": "3.03E-08", "module": "C3", "scenario": "S2"}, {"value": "4.081E-08", "module": "C3", "scenario": "S3"}, {"value": "2.458E-08", "module": "C4"}, {"value": "-3.934E-09", "module": "D", "scenario": "S0"}, {"value": "0", "module": "D", "scenario": "S1"}, {"value": "-5.656E-08", "module": "D", "scenario": "S2"}, {"value": "-3.734E-08", "module": "D", "scenario": "S3"}]}}, {"referenceToLCIAMethodDataSet": {"shortDescription": [{"value": "Abiotic depletion potential for fossil resources (ADPF)", "lang": "en"}, {"value": "Potenzial für den abiotischen Abbau fossiler Brennstoffe (ADPF)", "lang": "de"}], "type": "LCIA method data set", "refObjectId": "b2ad6110-c78d-11e6-9d9d-cec0c932ce01", "uri": "../lciamethods/b2ad6110-c78d-11e6-9d9d-cec0c932ce01.xml"}, "other": {"anies": [{"name": "referenceToUnitGroupDataSet", "value": {"shortDescription": [{"value": "MJ", "lang": "en"}], "type": "unit group data set", "refObjectId": "93a60a57-a3c8-11da-a746-0800200c9a66", "uri": "../unitgroups/93a60a57-a3c8-11da-a746-0800200c9a66.xml"}}, {"value": "127.8", "module": "A1-A3"}, {"value": "4.065", "module": "A4"}, {"value": "4.0737", "module": "A5"}, {"value": "0", "module": "B1"}, {"value": "4.5", "module": "B2"}, {"value": "0", "module": "C1"}, {"value": "0.2262", "module": "C2"}, {"value": "3.485", "module": "C3", "scenario": "S2"}, {"value": "4.515", "module": "C3", "scenario": "S3"}, {"value": "5.029", "module": "C4"}, {"value": "-0.4567", "module": "D", "scenario": "S0"}, {"value": "0", "module": "D", "scenario": "S1"}, {"value": "-6.847", "module": "D", "scenario": "S2"}, {"value": "-36.6", "module": "D", "scenario": "S3"}]}}, {"referenceToLCIAMethodDataSet": {"shortDescription": [{"value": "Water use (WDP)", "lang": "en"}, {"value": "Wassernutzung (WDP)", "lang": "de"}], "type": "LCIA method data set", "refObjectId": "b2ad66ce-c78d-11e6-9d9d-cec0c932ce01", "uri": "../lciamethods/b2ad66ce-c78d-11e6-9d9d-cec0c932ce01.xml"}, "other": {"anies": [{"name": "referenceToUnitGroupDataSet", "value": {"shortDescription": [{"value": "m^(3) world eq deprived", "lang": "en"}], "type": "unit group data set", "refObjectId": "6ae2df01-888e-46c8-b17d-49fa3869b476", "uri": "../unitgroups/6ae2df01-888e-46c8-b17d-49fa3869b476.xml"}}, {"value": "5.126", "module": "A1-A3"}, {"value": "0.002721", "module": "A4"}, {"value": "0.17952", "module": "A5"}, {"value": "0", "module": "B1"}, {"value": "0.07225", "module": "B2"}, {"value": "0", "module": "C1"}, {"value": "0.0001514", "module": "C2"}, {"value": "0.7587", "module": "C3", "scenario": "S2"}, {"value": "0.7649", "module": "C3", "scenario": "S3"}, {"value": "-0.00376", "module": "C4"}, {"value": "-0.002708", "module": "D", "scenario": "S0"}, {"value": "0", "module": "D", "scenario": "S1"}, {"value": "-0.03809", "module": "D", "scenario": "S2"}, {"value": "-0.04926", "module": "D", "scenario": "S3"}]}}, {"referenceToLCIAMethodDataSet": {"shortDescription": [{"value": "Incidence of disease due to PM emissions (PM)", "lang": "en"}, {"value": "Auftreten von Krankheiten aufgrund von Feinstaubemissionen (PM)", "lang": "de"}], "type": "LCIA method data set", "refObjectId": "b5c602c6-def3-11e6-bf01-fe55135034f3", "uri": "../lciamethods/b5c602c6-def3-11e6-bf01-fe55135034f3.xml"}, "other": {"anies": [{"name": "referenceToUnitGroupDataSet", "value": {"shortDescription": [{"value": "Disease incidence", "lang": "en"}], "type": "unit group data set", "refObjectId": "3883559b-648f-4afc-8ba2-0bd24f3affa3", "uri": "../unitgroups/3883559b-648f-4afc-8ba2-0bd24f3affa3.xml"}}, {"value": "1.51E-07", "module": "A1-A3"}, {"value": "1.05E-08", "module": "A4"}, {"value": "5.66E-09", "module": "A5"}, {"value": "0", "module": "B1"}, {"value": "4.27E-08", "module": "B2"}, {"value": "0", "module": "C1"}, {"value": "5.82E-10", "module": "C2"}, {"value": "2.58E-08", "module": "C3", "scenario": "S2"}, {"value": "2.78E-08", "module": "C3", "scenario": "S3"}, {"value": "1.01E-08", "module": "C4"}, {"value": "-2.86E-10", "module": "D", "scenario": "S0"}, {"value": "0", "module": "D", "scenario": "S1"}, {"value": "0", "module": "D", "scenario": "S2"}, {"value": "-3.94E-08", "module": "D", "scenario": "S3"}]}}, {"referenceToLCIAMethodDataSet": {"shortDescription": [{"value": "Human exposure efficiency relative to U235 (IR)", "lang": "en"}, {"value": "Wirkung durch Exposition des Menschen mit U235 (IR)", "lang": "de"}], "type": "LCIA method data set", "refObjectId": "b5c632be-def3-11e6-bf01-fe55135034f3", "uri": "../lciamethods/b5c632be-def3-11e6-bf01-fe55135034f3.xml"}, "other": {"anies": [{"name": "referenceToUnitGroupDataSet", "value": {"shortDescription": [{"value": "kBq U235 eq", "lang": "en"}], "type": "unit group data set", "refObjectId": "456b05bf-1415-44a9-9993-02452f554c09", "uri": "../unitgroups/456b05bf-1415-44a9-9993-02452f554c09.xml"}}, {"value": "0.41", "module": "A1-A3"}, {"value": "0.000736", "module": "A4"}, {"value": "0.012949", "module": "A5"}, {"value": "0", "module": "B1"}, {"value": "0.0658", "module": "B2"}, {"value": "0", "module": "C1"}, {"value": "4.09E-05", "module": "C2"}, {"value": "0.0196", "module": "C3", "scenario": "S2"}, {"value": "0.0323", "module": "C3", "scenario": "S3"}, {"value": "0.00912", "module": "C4"}, {"value": "-0.00583", "module": "D", "scenario": "S0"}, {"value": "0", "module": "D", "scenario": "S1"}, {"value": "0", "module": "D", "scenario": "S2"}, {"value": "-0.015", "module": "D", "scenario": "S3"}]}}, {"referenceToLCIAMethodDataSet": {"shortDescription": [{"value": "Comparative toxic unit for ecosystems (ETP-fw)", "lang": "en"}, {"value": "Toxizitätsvergleichseinheit für Ökosysteme (ETP-fw)", "lang": "de"}], "type": "LCIA method data set", "refObjectId": "ee1082d1-b0f7-43ca-a1f0-21e2a4a74511", "uri": "../lciamethods/ee1082d1-b0f7-43ca-a1f0-21e2a4a74511.xml"}, "other": {"anies": [{"name": "referenceToUnitGroupDataSet", "value": {"shortDescription": [{"value": "CTUe", "lang": "en"}], "type": "unit group data set", "refObjectId": "aa959ded-f1eb-4efb-9c5c-2d60be36b3e6", "uri": "../unitgroups/aa959ded-f1eb-4efb-9c5c-2d60be36b3e6.xml"}}, {"value": "63.3", "module": "A1-A3"}, {"value": "2.82", "module": "A4"}, {"value": "2.049", "module": "A5"}, {"value": "0.0036", "module": "B1"}, {"value": "2.03", "module": "B2"}, {"value": "0", "module": "C1"}, {"value": "0.157", "module": "C2"}, {"value": "1.9", "module": "C3", "scenario": "S2"}, {"value": "2.5", "module": "C3", "scenario": "S3"}, {"value": "4.92", "module": "C4"}, {"value": "-0.0961", "module": "D", "scenario": "S0"}, {"value": "0", "module": "D", "scenario": "S1"}, {"value": "0", "module": "D", "scenario": "S2"}, {"value": "-6.86", "module": "D", "scenario": "S3"}]}}, {"referenceToLCIAMethodDataSet": {"shortDescription": [{"value": "Comparative toxic unit for humans (carcinogenic) (HTP-c)", "lang": "en"}, {"value": "Toxizitätsvergleichseinheit für Menschen (krebserregend) (HTP-c)", "lang": "de"}], "type": "LCIA method data set", "refObjectId": "2299222a-bbd8-474f-9d4f-4dd1f18aea7c", "uri": "../lciamethods/2299222a-bbd8-474f-9d4f-4dd1f18aea7c.xml"}, "other": {"anies": [{"name": "referenceToUnitGroupDataSet", "value": {"shortDescription": [{"value": "CTUh", "lang": "en"}], "type": "unit group data set", "refObjectId": "d4c9523e-2d7e-49fd-8469-998f547d3a70", "uri": "../unitgroups/d4c9523e-2d7e-49fd-8469-998f547d3a70.xml"}}, {"value": "2.76E-09", "module": "A1-A3"}, {"value": "5.71E-11", "module": "A4"}, {"value": "8.751E-11", "module": "A5"}, {"value": "0", "module": "B1"}, {"value": "3.9E-10", "module": "B2"}, {"value": "0", "module": "C1"}, {"value": "3.17E-12", "module": "C2"}, {"value": "8.89E-11", "module": "C3", "scenario": "S2"}, {"value": "1.03E-10", "module": "C3", "scenario": "S3"}, {"value": "2.21E-10", "module": "C4"}, {"value": "-4.56E-12", "module": "D", "scenario": "S0"}, {"value": "0", "module": "D", "scenario": "S1"}, {"value": "0", "module": "D", "scenario": "S2"}, {"value": "-1E-10", "module": "D", "scenario": "S3"}]}}, {"referenceToLCIAMethodDataSet": {"shortDescription": [{"value": "Comparative toxic unit for humans (noncarcinogenic) (HTP-nc)", "lang": "en"}, {"value": "Toxizitätsvergleichseinheit für Menschen (nicht krebserregend) (HTP-nc)", "lang": "de"}], "type": "LCIA method data set", "refObjectId": "3af763a5-b7a1-48c9-9cee-1f223481fcef", "uri": "../lciamethods/3af763a5-b7a1-48c9-9cee-1f223481fcef.xml"}, "other": {"anies": [{"name": "referenceToUnitGroupDataSet", "value": {"shortDescription": [{"value": "CTUh", "lang": "en"}], "type": "unit group data set", "refObjectId": "d4c9523e-2d7e-49fd-8469-998f547d3a70", "uri": "../unitgroups/d4c9523e-2d7e-49fd-8469-998f547d3a70.xml"}}, {"value": "1.02E-07", "module": "A1-A3"}, {"value": "3.38E-09", "module": "A4"}, {"value": "3.372E-09", "module": "A5"}, {"value": "2.6E-11", "module": "B1"}, {"value": "6.19E-09", "module": "B2"}, {"value": "0", "module": "C1"}, {"value": "1.88E-10", "module": "C2"}, {"value": "6.55E-09", "module": "C3", "scenario": "S2"}, {"value": "7.24E-09", "module": "C3", "scenario": "S3"}, {"value": "1.85E-08", "module": "C4"}, {"value": "-1.76E-10", "module": "D", "scenario": "S0"}, {"value": "0", "module": "D", "scenario": "S1"}, {"value": "0", "module": "D", "scenario": "S2"}, {"value": "-6.52E-09", "module": "D", "scenario": "S3"}]}}, {"referenceToLCIAMethodDataSet": {"shortDescription": [{"value": "Soil quality index (SQP)", "lang": "en"}, {"value": "Bodenqualitätsindex (SQP)", "lang": "de"}], "type": "LCIA method data set", "refObjectId": "b2ad6890-c78d-11e6-9d9d-cec0c932ce01", "uri": "../lciamethods/b2ad6890-c78d-11e6-9d9d-cec0c932ce01.xml"}, "other": {"anies": [{"name": "referenceToUnitGroupDataSet", "value": {"shortDescription": [{"value": "SQP", "lang": "en"}], "type": "unit group data set", "refObjectId": "f130951c-e67f-4f7f-8dd4-665de3974e18", "uri": "../unitgroups/f130951c-e67f-4f7f-8dd4-665de3974e18.xml"}}, {"module": "A1-A3"}, {"module": "A4"}, {"module": "A5"}, {"module": "B1"}, {"module": "B2"}, {"module": "C1"}, {"module": "C2"}, {"module": "C3", "scenario": "S2"}, {"module": "C3", "scenario": "S3"}, {"module": "C4"}, {"module": "D", "scenario": "S0"}, {"module": "D", "scenario": "S1"}, {"module": "D", "scenario": "S2"}, {"module": "D", "scenario": "S3"}]}}]}, "otherAttributes": {"{http://www.indata.network/EPD/2019}epd-version": "1.2"}, "version": "1.1", "locations": "../ILCDLocations.xml"}