{"processInformation": {"dataSetInformation": {"UUID": "d314e372-23b2-44fd-9b82-e503815cbbf2", "name": {"baseName": [{"value": "Kentaur", "lang": "en"}, {"value": "Kentaur", "lang": "de"}], "functionalUnitFlowProperties": [{"lang": "en"}]}, "classificationInformation": {"classification": [{"class": [{"value": "Komponenten von Fenstern und Vorhangfassaden", "level": 0, "classId": "7"}, {"value": "Türen und Tore", "level": 1, "classId": "7.6"}, {"value": "Stahl", "level": 2, "classId": "7.6.01"}], "name": "OEKOBAU.DAT"}, {"class": [{"value": "02 Building products", "level": 0}, {"value": "Doors, windows, shutters, and related products", "level": 1}, {"value": "Electronic and physical Access Control Systems", "level": 2}], "name": "IBUCategories"}]}, "generalComment": [{"value": "The robust Kentaur Full-Height Turnstiles are especially suitable for securing the perimeter of buildings and property.\nVersatile versions enable individual combinations of multiple units to be put together. The end point locking system developed by dormakaba prevents people from being trapped in the gates.\n\nVersatility\nThe Kentaur product series offers a modular design. Two, three and four-winged units with straight or U-shaped bars can be combined with each other. The same applies for units with bicycle doors, integrated doors, an emergency exit function of resistance class RC2. The roofs fit with any of the single, multiple or space-saving double units.\n\nMinimal power consumption\nThe low-energy drive consumes little energy.\n\nSafe passage\nThe end point locking implemented in Kentaur turnstiles prevents people from becoming trapped or jammed. After release the turnstile may be stopped at any time and rotated backwards as long as it has not yet completed half of its rotation.\nOnce the turnstile has completed half of its rotary motion, the unit can only be exited in the released direction.", "lang": "en"}, {"value": "Die robusten Kentaur Full-Height Drehkreuze eignen sich besonders für die Absicherung von Gebäude- und Grundstücksgrenzen. Vielseitige Ausführungen ermöglichen die individuelle Zusammenstellung von mehreren Einheiten. Das von dormakaba entwickelte Endpunktverriegelungssystem verhindert, dass Personen in den Toren eingeklemmt werden. Vielseitigkeit Die Kentaur Produktserie ist modular aufgebaut. Zwei-, drei- und vierflügelige Einheiten mit geraden oder U-förmigen Stäben können miteinander kombiniert werden. Das Gleiche gilt für Einheiten mit Fahrradtüren, integrierten Türen, einer Notausgangsfunktion der Widerstandsklasse RC2. Die Dächer passen zu jeder der Einzel-, Mehrfach- oder platzsparenden Doppeleinheiten. Minimaler Stromverbrauch Der Niedrigenergieantrieb verbraucht wenig Energie. Sicherer Durchgang Die in Kentaur-Drehkreuzen implementierte Endpunktverriegelung verhindert, dass Personen eingeklemmt werden oder stecken bleiben. Nach der Freigabe kann das Drehkreuz jederzeit angehalten und rückwärts gedreht werden, solange es noch nicht die Hälfte seiner Drehbewegung vollendet hat. Sobald das Drehkreuz die Hälfte seiner Drehbewegung vollendet hat, kann die Einheit nur noch in der freigegebenen Richtung verlassen werden.", "lang": "de"}]}, "quantitativeReference": {"referenceToReferenceFlow": [0]}, "time": {"referenceYear": 2022, "dataSetValidUntil": 2027, "other": {"anies": [{"name": "publicationDateOfEPD", "value": 1665964800000}]}}, "geography": {"locationOfOperationSupplyOrProduction": {"location": "DE"}}, "technology": {"technologyDescriptionAndIncludedProcesses": [{"value": "The robust Kentaur full-height turnstiles are particularly suitable for securing building and property boundaries. Versatile designs enable the individual combination of several units. The end-point locking system developed by dormakaba prevents people from becoming trapped in the gates. \nTechnical data: \nFollowing technical data apply for the Kentaur Full-Height Turnstile (FTS-E02): \nDeclared unit: \nThe declared unit is 1 piece of product: 302,95 kg", "lang": "en"}, {"value": "Die robusten Kentaur Full-Height Drehkreuze eignen sich besonders für die Absicherung von Gebäude- und Grundstücksgrenzen.\nVielseitige Ausführungen ermöglichen die individuelle Zusammenstellung mehrerer Einheiten. Die von dormakaba entwickelte Endpunktverriegelung verhindert, dass Personen in den Toren eingeklemmt werden. \nTechnische Daten: \nDie folgenden technischen Daten gelten für das Kentaur Full-Height Turnstile (FTS-E02): \nDeklarierte Einheit: \nDie angegebene Einheit ist 1 Stück des Produkts: 302,95 kg", "lang": "de"}], "technologicalApplicability": [{"value": "For reliabable security at:\n\nManufacturing plants\nCompany sites\nAirports and ports\nPower plants\nCar parks\nBicycle stands\nCorrectional facilities\nMilitary installations\nEducational centres\nStadiums\nAmusement parks", "lang": "en"}, {"value": "Für verlässliche Sicherheit bei:\n· Produktionsstätten\n· Firmengeländen\n· Flughäfen und Häfen\n· Kraftwerken\n· Parkhäusern\n· Fahrradständer\n· Justizvollzugsanstalten\n· Militärische Einrichtungen\n· Bildungszentren\n· Stadien\n· Vergnügungsparks", "lang": "de"}]}}, "modellingAndValidation": {"LCIMethodAndAllocation": {"typeOfDataSet": "EPD", "referenceToLCAMethodDetails": [{"shortDescription": [{"value": "Electronic and physical Access Control Systems.pdf", "lang": "en"}], "type": "source data set", "refObjectId": "7cb4d0b2-0a27-446c-99b5-9998abf0714b"}], "other": {"anies": [{"name": "subType", "value": "specific dataset"}]}}, "dataSourcesTreatmentAndRepresentativeness": {"referenceToDataSource": [{"shortDescription": [{"value": "GaBi Database (all versions)", "lang": "en"}], "type": "source data set", "refObjectId": "28d74cc0-db8b-4d7e-bc44-5f6d56ce0c4a"}, {"shortDescription": [{"value": "GaBi Database Edition 2021, CUP 2021.01", "lang": "en"}], "type": "source data set", "refObjectId": "1cece811-7501-44d4-8067-9259bd5cb835"}], "useAdviceForDataSet": [{"value": "Scope: \nThis EPD is a specific product declaration for the Kentaur Full-Height Turnstiles (FTS-E02).\nThe underlying life cycle assessment is based on the entire life cycle of this specific Kentaur Full-Height Turnstile.\nThe products are manufactured at the dormakaba production facility in Bhl (Germany).\nGreen electricity is being used at this production site.\n\nData represents the year 2022. \nSystem boundary: \nType of EPD: cradle to gate with options, modules C1–C4, and module D (A1–A3 + C + D and additional modules: A4 + A5 + B6)\n\nProduction - Module A1-A3\nThe product stage includes:\n— A1, raw material extraction, processing and mechanical treatments, processing of secondary material input (e.g. recycling processes),\n— A2, transport to the manufacturer,\n— A3, manufacturing and assembly including provision of all materials, products and energy, as well as waste processing up to the end-of waste state.\n\nConstruction stage - Modules A4-A5\nThe construction process stage includes:\n— A4, transport to the building site;\n— A5, installation into the building;\nincluding provision of all materials, products and energy, as well as waste processing up to the end-of-waste state or disposal of final residues during the construction process stage.\n\nUse stage - Module B6\nThe use stage related to the operation of the building includes:\n— B6, operational energy use\nThe potential use of electricity from the grid is declared in module B6.\n\nEnd-of-life stage– Modules C1-C4 and D\nThe end-of-life stage includes:\n— C1, de-construction, demolition:\n— C2, transport to waste processing;\n— C3, waste processing for reuse, recovery and/or recycling;\n— C4, disposal;\nincluding provision and all transport, provision of all materials, products and related energy and water use.\n\nModule D (Benefits and loads beyond the system boundary) includes:\n— D, recycling potentials, expressed as net impacts and benefits.", "lang": "en"}, {"value": "Gültigkeitsbereich: \nDiese EPD ist eine spezifische Produktdeklaration für das Kentaur Full-Height Drehkreuz (FTS-E02). Die zugrundeliegende Ökobilanz basiert auf dem gesamten Lebenszyklus dieses spezifischen Kentaur Full-Height Drehkreuzes. Die Produkte werden in der dormakaba Produktionsstätte in Bühl (Deutschland) hergestellt. An diesem Produktionsstandort wird Ökostrom verwendet. Die Daten beziehen sich auf das Jahr 2022. \nSystemgrenze: \nArt der EPD: Cradle to Gate mit Optionen, Modulen C1-C4 und Modul D (A1-A3 + C + D und zusätzliche Module: A4 + A5 + B6) Produktion - Modul A1-A3 Die Produktphase umfasst: - A1, Rohstoffgewinnung, Verarbeitung und mechanische Behandlungen, Verarbeitung von Sekundärmaterial-Input (z.B. Recyclingprozesse), - A2, Transport zum Hersteller, - A3, Herstellung und Montage einschließlich Bereitstellung aller Materialien, Produkte und Energie sowie Abfallverarbeitung bis zum End-of-Waste-Zustand.\n\n\n\nBauphase - Module A4-A5 Die Bauprozessphase umfasst: - A4, Transport zur Baustelle; - A5, Einbau in das Gebäude; einschließlich der Bereitstellung aller Materialien, Produkte und Energie sowie der Abfallverarbeitung bis zum Abfallende oder der Entsorgung der letzten Rückstände während der Bauprozessphase.\n \n\nNutzungsphase - Modul B6 Die Nutzungsphase im Zusammenhang mit dem Betrieb des Gebäudes umfasst: - B6, Betriebliche Energienutzung Die potenzielle Nutzung von Strom aus dem Netz wird in Modul B6 angegeben.\n\n\n \n\n\nEnd-of-Life-Phase - Module C1-C4 und D Die End-of-Life-Phase umfasst: - C1, Rückbau, Abriss; - C2, Transport zur Abfallverarbeitung; - C3, Abfallverarbeitung zur Wiederverwendung, Rückgewinnung und/oder zum Recycling; - C4, Entsorgung; einschließlich Bereitstellung und sämtlicher Transporte, Bereitstellung aller Materialien, Produkte und des damit verbundenen Energie- und Wasserverbrauchs. Modul D (Nutzen und Belastungen jenseits der Systemgrenze) umfasst: - D, Recyclingpotenziale, ausgedrückt als Nettoauswirkungen und Nutzen.", "lang": "de"}], "other": {"anies": [{"name": "referenceToOriginalEPD", "value": {"shortDescription": {"value": "Kentaur.pdf", "defaultValue": "Kentaur.pdf", "lstrings": [{"lang": "en", "value": "Kentaur.pdf"}]}, "type": "source data set", "uuid": {"uuid": "b3a980a5-d634-45f0-82dc-9fa8dd20ba2b"}, "refObjectId": "b3a980a5-d634-45f0-82dc-9fa8dd20ba2b", "resourceURLs": ["https://oekobaudat.de/OEKOBAU.DAT/resource/sources/b3a980a5-d634-45f0-82dc-9fa8dd20ba2b/Kentaur_22676.pdf?version=00.05.000"]}}]}}, "validation": {"review": [{"referenceToNameOfReviewerAndInstitution": [{"shortDescription": [{"value": "Institut Bauen und Umwelt e. V.", "lang": "en"}], "type": "contact data set", "refObjectId": "d111dbec-b024-4be5-86c5-752d6eb2cf95", "uri": "../contacts/d111dbec-b024-4be5-86c5-752d6eb2cf95.xml"}], "type": "Accredited third party review"}]}, "complianceDeclarations": {"compliance": [{"referenceToComplianceSystem": {"shortDescription": [{"value": "DIN EN 15804+A2", "lang": "en"}], "type": "source data set", "refObjectId": "c0016b33-8cf7-415c-ac6e-deba0d21440d", "uri": "../sources/c0016b33-8cf7-415c-ac6e-deba0d21440d.xml"}}, {"referenceToComplianceSystem": {"shortDescription": [{"value": "ISO 14025", "lang": "en"}], "type": "source data set", "refObjectId": "4f2eb655-6e44-4874-a95a-e28f5442cd4d", "uri": "../sources/4f2eb655-6e44-4874-a95a-e28f5442cd4d.xml"}}]}}, "administrativeInformation": {"commissionerAndGoal": {"referenceToCommissioner": [{"shortDescription": [{"value": "dormakaba International Holding GmbH", "lang": "en"}], "type": "contact data set", "refObjectId": "33313944-7b37-498a-b458-25a295c1017d", "uri": "../contacts/33313944-7b37-498a-b458-25a295c1017d.xml"}]}, "dataGenerator": {"referenceToPersonOrEntityGeneratingTheDataSet": [{"shortDescription": [{"value": "Sphera Solutions GmbH", "lang": "en"}], "type": "contact data set", "refObjectId": "623edf96-39d1-4e6f-9892-674c7228546b", "uri": "../contacts/623edf96-39d1-4e6f-9892-674c7228546b.xml"}]}, "dataEntryBy": {"timeStamp": 1665964800000, "referenceToDataSetFormat": [{"shortDescription": [{"value": "ILCD Format", "lang": "en"}], "type": "source data set", "refObjectId": "a97a0155-0234-4b87-b4ce-a45da52f2a40", "uri": "../sources/a97a0155-0234-4b87-b4ce-a45da52f2a40.xml"}, {"shortDescription": [{"value": "EPD-Datenformaterweiterungen v1.2", "lang": "de"}, {"value": "EPD Data Format Extensions v1.2", "lang": "en"}], "type": "source data set", "refObjectId": "a29449fd-aa2f-4de8-b5d7-4b06b43c6fde", "uri": "../sources/a29449fd-aa2f-4de8-b5d7-4b06b43c6fde.xml"}]}, "publicationAndOwnership": {"dataSetVersion": "00.06.100", "referenceToRegistrationAuthority": {"shortDescription": [{"value": "Institut Bauen und Umwelt e. V.", "lang": "en"}], "type": "contact data set", "refObjectId": "d111dbec-b024-4be5-86c5-752d6eb2cf95", "uri": "../contacts/d111dbec-b024-4be5-86c5-752d6eb2cf95.xml"}, "registrationNumber": "EPD-DOR-20220166-CBA1-EN", "referenceToOwnershipOfDataSet": {"shortDescription": [{"value": "dormakaba International Holding GmbH", "lang": "en"}], "type": "contact data set", "refObjectId": "33313944-7b37-498a-b458-25a295c1017d", "uri": "../contacts/33313944-7b37-498a-b458-25a295c1017d.xml"}, "copyright": true, "licenseType": "Free of charge for all users and uses", "accessRestrictions": [{"value": "None", "lang": "en"}], "other": {"anies": [{"name": "referenceToPublisher", "value": {"shortDescription": [{"value": "Institut Bauen und Umwelt e. V.", "lang": "en"}], "type": "contact data set", "refObjectId": "d111dbec-b024-4be5-86c5-752d6eb2cf95", "uri": "../contacts/d111dbec-b024-4be5-86c5-752d6eb2cf95.xml"}}]}}}, "exchanges": {"exchange": [{"dataSetInternalID": 0, "referenceToFlowDataSet": {"shortDescription": [{"value": "Kentaur (Kentaur)", "lang": "en"}], "type": "flow data set", "refObjectId": "b771c50f-060f-9e6f-48a5-8e7f4c9d2053", "uri": "../flows/b771c50f-060f-9e6f-48a5-8e7f4c9d2053.xml"}, "meanAmount": 1.0, "referencesToDataSource": {}, "referenceFlow": true, "resolvedFlowVersion": "00.06.100", "resultingflowAmount": 1.0, "flowProperties": [{"name": [{"lang": "en", "value": "Weight"}], "uuid": "93a60a56-a3c8-11da-a746-0800200b9a66", "meanValue": 306.49}, {"name": [{"lang": "de", "value": "Anzahl"}, {"lang": "en", "value": "Number of pieces"}], "uuid": "01846770-4cfe-4a25-8ad9-919d8d378345", "referenceFlowProperty": true, "meanValue": 1.0, "referenceUnit": "pcs.", "unitGroupUUID": "934110e3-baf4-49e9-992c-3d8109a6aafb"}], "materialProperties": [{"name": "weight per piece", "value": "306.49", "unit": "kg"}], "typeOfFlow": "Product flow", "classification": {"classHierarchy": "Komponenten von Fenstern und Vorhangfassaden / Türen und Tore / Stahl", "name": "OEKOBAU.DAT"}}, {"dataSetInternalID": 1, "referenceToFlowDataSet": {"shortDescription": [{"value": "Renewable primary energy as energy carrier (PERE)", "lang": "en"}, {"value": "Erneuerbare Primärenergie als Energieträger (PERE)", "lang": "de"}], "type": "flow data set", "refObjectId": "20f32be5-0398-4288-9b6d-accddd195317", "uri": "../flows/20f32be5-0398-4288-9b6d-accddd195317.xml"}, "exchange direction": "INPUT", "other": {"anies": [{"name": "referenceToUnitGroupDataSet", "value": {"shortDescription": [{"value": "MJ", "lang": "en"}], "type": "unit group data set", "refObjectId": "93a60a57-a3c8-11da-a746-0800200c9a66", "uri": "../unitgroups/93a60a57-a3c8-11da-a746-0800200c9a66.xml"}}, {"value": "2571.087", "module": "A1-A3"}, {"value": "0.115", "module": "A4"}, {"value": "12.281", "module": "A5"}, {"value": "0", "module": "B2"}, {"value": "4362", "module": "B6"}, {"value": "0", "module": "C1"}, {"value": "0.057", "module": "C2"}, {"value": "14.532", "module": "C3"}, {"value": "1.324", "module": "C4"}, {"value": "-932.64", "module": "D"}]}, "resolvedFlowVersion": "38.00.000", "flowProperties": [], "typeOfFlow": "Other flow", "classification": {"classHierarchy": "Quantities", "name": "GaBiCategories"}}, {"dataSetInternalID": 2, "referenceToFlowDataSet": {"shortDescription": [{"value": "Renewable primary energy resources as material utilization (PERM)", "lang": "en"}, {"value": "Erneuerbare Primärenergie zur stofflichen Nutzung (PERM)", "lang": "de"}], "type": "flow data set", "refObjectId": "fb3ec0de-548d-4508-aea5-00b73bf6f702", "uri": "../flows/fb3ec0de-548d-4508-aea5-00b73bf6f702.xml"}, "exchange direction": "INPUT", "other": {"anies": [{"name": "referenceToUnitGroupDataSet", "value": {"shortDescription": [{"value": "MJ", "lang": "en"}], "type": "unit group data set", "refObjectId": "93a60a57-a3c8-11da-a746-0800200c9a66", "uri": "../unitgroups/93a60a57-a3c8-11da-a746-0800200c9a66.xml"}}, {"value": "25.32", "module": "A1-A3"}, {"value": "0", "module": "A4"}, {"value": "-12", "module": "A5"}, {"value": "0", "module": "B2"}, {"value": "0", "module": "B6"}, {"value": "0", "module": "C1"}, {"value": "0", "module": "C2"}, {"value": "-13.32", "module": "C3"}, {"value": "0", "module": "C4"}, {"value": "0", "module": "D"}]}, "resolvedFlowVersion": "38.00.000", "flowProperties": [], "typeOfFlow": "Other flow", "classification": {"classHierarchy": "Quantities", "name": "GaBiCategories"}}, {"dataSetInternalID": 3, "referenceToFlowDataSet": {"shortDescription": [{"value": "Total use of renewable primary energy resources (PERT)", "lang": "en"}, {"value": "Total erneuerbare Primärenergie (PERT)", "lang": "de"}], "type": "flow data set", "refObjectId": "53f97275-fa8a-4cdd-9024-65936002acd0", "uri": "../flows/53f97275-fa8a-4cdd-9024-65936002acd0.xml"}, "exchange direction": "INPUT", "other": {"anies": [{"name": "referenceToUnitGroupDataSet", "value": {"shortDescription": [{"value": "MJ", "lang": "en"}], "type": "unit group data set", "refObjectId": "93a60a57-a3c8-11da-a746-0800200c9a66", "uri": "../unitgroups/93a60a57-a3c8-11da-a746-0800200c9a66.xml"}}, {"value": "2596.387", "module": "A1-A3"}, {"value": "0.115", "module": "A4"}, {"value": "0.281", "module": "A5"}, {"value": "0", "module": "B2"}, {"value": "4362", "module": "B6"}, {"value": "0", "module": "C1"}, {"value": "0.057", "module": "C2"}, {"value": "1.212", "module": "C3"}, {"value": "1.324", "module": "C4"}, {"value": "-932.64", "module": "D"}]}, "resolvedFlowVersion": "38.00.000", "flowProperties": [], "typeOfFlow": "Other flow", "classification": {"classHierarchy": "Quantities / Environmental quantities / EPD EN 15804 / LCI indicators", "name": "GaBiCategories"}}, {"dataSetInternalID": 4, "referenceToFlowDataSet": {"shortDescription": [{"value": "Non renewable primary energy as energy carrier (PENRE)", "lang": "en"}, {"value": "Nicht-erneuerbare Primärenergie als Energieträger (PENRE)", "lang": "de"}], "type": "flow data set", "refObjectId": "ac857178-2b45-46ec-892a-a9a4332f0372", "uri": "../flows/ac857178-2b45-46ec-892a-a9a4332f0372.xml"}, "exchange direction": "INPUT", "other": {"anies": [{"name": "referenceToUnitGroupDataSet", "value": {"shortDescription": [{"value": "MJ", "lang": "en"}], "type": "unit group data set", "refObjectId": "93a60a57-a3c8-11da-a746-0800200c9a66", "uri": "../unitgroups/93a60a57-a3c8-11da-a746-0800200c9a66.xml"}}, {"value": "8652.11", "module": "A1-A3"}, {"value": "36.369", "module": "A4"}, {"value": "29.164", "module": "A5"}, {"value": "0", "module": "B2"}, {"value": "9843.2", "module": "B6"}, {"value": "0", "module": "C1"}, {"value": "18.172", "module": "C2"}, {"value": "159.83", "module": "C3"}, {"value": "10.113", "module": "C4"}, {"value": "-3659.7", "module": "D"}]}, "resolvedFlowVersion": "38.00.000", "flowProperties": [], "typeOfFlow": "Other flow", "classification": {"classHierarchy": "Quantities", "name": "GaBiCategories"}}, {"dataSetInternalID": 5, "referenceToFlowDataSet": {"shortDescription": [{"value": "Non renewable primary energy as material utilization (PENRM)", "lang": "en"}, {"value": "Nicht-erneuerbare Primärenergie zur stofflichen Nutzung (PENRM)", "lang": "de"}], "type": "flow data set", "refObjectId": "1421caa0-679d-4bf4-b282-0eb850ccae27", "uri": "../flows/1421caa0-679d-4bf4-b282-0eb850ccae27.xml"}, "exchange direction": "INPUT", "other": {"anies": [{"name": "referenceToUnitGroupDataSet", "value": {"shortDescription": [{"value": "MJ", "lang": "en"}], "type": "unit group data set", "refObjectId": "93a60a57-a3c8-11da-a746-0800200c9a66", "uri": "../unitgroups/93a60a57-a3c8-11da-a746-0800200c9a66.xml"}}, {"value": "183", "module": "A1-A3"}, {"value": "0", "module": "A4"}, {"value": "-27.95", "module": "A5"}, {"value": "0", "module": "B2"}, {"value": "0", "module": "B6"}, {"value": "0", "module": "C1"}, {"value": "0", "module": "C2"}, {"value": "-155.05", "module": "C3"}, {"value": "0", "module": "C4"}, {"value": "0", "module": "D"}]}, "resolvedFlowVersion": "38.00.000", "flowProperties": [], "typeOfFlow": "Other flow", "classification": {"classHierarchy": "Quantities", "name": "GaBiCategories"}}, {"dataSetInternalID": 6, "referenceToFlowDataSet": {"shortDescription": [{"value": "Total use of non renewable primary energy resources (PENRT)", "lang": "en"}, {"value": "Total nicht erneuerbare Primärenergie (PENRT)", "lang": "de"}], "type": "flow data set", "refObjectId": "06159210-646b-4c8d-8583-da9b3b95a6c1", "uri": "../flows/06159210-646b-4c8d-8583-da9b3b95a6c1.xml"}, "exchange direction": "INPUT", "other": {"anies": [{"name": "referenceToUnitGroupDataSet", "value": {"shortDescription": [{"value": "MJ", "lang": "en"}], "type": "unit group data set", "refObjectId": "93a60a57-a3c8-11da-a746-0800200c9a66", "uri": "../unitgroups/93a60a57-a3c8-11da-a746-0800200c9a66.xml"}}, {"value": "8835.11", "module": "A1-A3"}, {"value": "36.369", "module": "A4"}, {"value": "1.214", "module": "A5"}, {"value": "0", "module": "B2"}, {"value": "9843.2", "module": "B6"}, {"value": "0", "module": "C1"}, {"value": "18.172", "module": "C2"}, {"value": "4.785", "module": "C3"}, {"value": "10.113", "module": "C4"}, {"value": "-3659.7", "module": "D"}]}, "resolvedFlowVersion": "38.00.000", "flowProperties": [], "typeOfFlow": "Other flow", "classification": {"classHierarchy": "Quantities / Environmental quantities / EPD EN 15804 / LCI indicators", "name": "GaBiCategories"}}, {"dataSetInternalID": 7, "referenceToFlowDataSet": {"shortDescription": [{"value": "Use of secondary material (SM)", "lang": "en"}, {"value": "Einsatz von Sekundärstoffen (SM)", "lang": "de"}], "type": "flow data set", "refObjectId": "c6a1f35f-2d09-4f54-8dfb-97e502e1ce92", "uri": "../flows/c6a1f35f-2d09-4f54-8dfb-97e502e1ce92.xml"}, "exchange direction": "INPUT", "other": {"anies": [{"name": "referenceToUnitGroupDataSet", "value": {"shortDescription": [{"value": "kg", "lang": "en"}], "type": "unit group data set", "refObjectId": "ad38d542-3fe9-439d-9b95-2f5f7752acaf", "uri": "../unitgroups/ad38d542-3fe9-439d-9b95-2f5f7752acaf.xml"}}, {"value": "228.04", "module": "A1-A3"}, {"value": "0", "module": "A4"}, {"value": "0", "module": "A5"}, {"value": "0", "module": "B2"}, {"value": "0", "module": "B6"}, {"value": "0", "module": "C1"}, {"value": "0", "module": "C2"}, {"value": "0", "module": "C3"}, {"value": "0", "module": "C4"}, {"value": "0", "module": "D"}]}, "resolvedFlowVersion": "38.00.000", "flowProperties": [], "typeOfFlow": "Other flow", "classification": {"classHierarchy": "Quantities / Environmental quantities / EPD EN 15804 / LCI indicators", "name": "GaBiCategories"}}, {"dataSetInternalID": 8, "referenceToFlowDataSet": {"shortDescription": [{"value": "Use of renewable secondary fuels (RSF)", "lang": "en"}, {"value": "Erneuerbare Sekundärbrennstoffe (RSF)", "lang": "de"}], "type": "flow data set", "refObjectId": "64333088-a55f-4aa2-9a31-c10b07816787", "uri": "../flows/64333088-a55f-4aa2-9a31-c10b07816787.xml"}, "exchange direction": "INPUT", "other": {"anies": [{"name": "referenceToUnitGroupDataSet", "value": {"shortDescription": [{"value": "MJ", "lang": "en"}], "type": "unit group data set", "refObjectId": "93a60a57-a3c8-11da-a746-0800200c9a66", "uri": "../unitgroups/93a60a57-a3c8-11da-a746-0800200c9a66.xml"}}, {"value": "0", "module": "A1-A3"}, {"value": "0", "module": "A4"}, {"value": "0", "module": "A5"}, {"value": "0", "module": "B2"}, {"value": "0", "module": "B6"}, {"value": "0", "module": "C1"}, {"value": "0", "module": "C2"}, {"value": "0", "module": "C3"}, {"value": "0", "module": "C4"}, {"value": "0", "module": "D"}]}, "resolvedFlowVersion": "38.00.000", "flowProperties": [], "typeOfFlow": "Other flow", "classification": {"classHierarchy": "Quantities / Environmental quantities / EPD EN 15804 / LCI indicators", "name": "GaBiCategories"}}, {"dataSetInternalID": 9, "referenceToFlowDataSet": {"shortDescription": [{"value": "Use of non renewable secondary fuels (NRSF)", "lang": "en"}, {"value": "Nicht erneuerbare Sekundärbrennstoffe (NRSF)", "lang": "de"}], "type": "flow data set", "refObjectId": "89def144-d39a-4287-b86f-efde453ddcb2", "uri": "../flows/89def144-d39a-4287-b86f-efde453ddcb2.xml"}, "exchange direction": "INPUT", "other": {"anies": [{"name": "referenceToUnitGroupDataSet", "value": {"shortDescription": [{"value": "MJ", "lang": "en"}], "type": "unit group data set", "refObjectId": "93a60a57-a3c8-11da-a746-0800200c9a66", "uri": "../unitgroups/93a60a57-a3c8-11da-a746-0800200c9a66.xml"}}, {"value": "0", "module": "A1-A3"}, {"value": "0", "module": "A4"}, {"value": "0", "module": "A5"}, {"value": "0", "module": "B2"}, {"value": "0", "module": "B6"}, {"value": "0", "module": "C1"}, {"value": "0", "module": "C2"}, {"value": "0", "module": "C3"}, {"value": "0", "module": "C4"}, {"value": "0", "module": "D"}]}, "resolvedFlowVersion": "38.00.000", "flowProperties": [], "typeOfFlow": "Other flow", "classification": {"classHierarchy": "Quantities / Environmental quantities / EPD EN 15804 / LCI indicators", "name": "GaBiCategories"}}, {"dataSetInternalID": 10, "referenceToFlowDataSet": {"shortDescription": [{"value": "Use of net fresh water (FW)", "lang": "en"}, {"value": "Einsatz von Süßwasserressourcen (FW)", "lang": "de"}], "type": "flow data set", "refObjectId": "3cf952c8-f3a4-461d-8c96-96456ca62246", "uri": "../flows/3cf952c8-f3a4-461d-8c96-96456ca62246.xml"}, "exchange direction": "INPUT", "other": {"anies": [{"name": "referenceToUnitGroupDataSet", "value": {"shortDescription": [{"value": "m^3", "lang": "en"}], "type": "unit group data set", "refObjectId": "cd950537-0a98-4044-9ba7-9f9a68d0a504", "uri": "../unitgroups/cd950537-0a98-4044-9ba7-9f9a68d0a504.xml"}}, {"value": "7.7937663", "module": "A1-A3"}, {"value": "0.0002055", "module": "A4"}, {"value": "0.008", "module": "A5"}, {"value": "0", "module": "B2"}, {"value": "5.044", "module": "B6"}, {"value": "0", "module": "C1"}, {"value": "0.0001027", "module": "C2"}, {"value": "0.028", "module": "C3"}, {"value": "0.003", "module": "C4"}, {"value": "-4.481", "module": "D"}]}, "resolvedFlowVersion": "38.00.000", "flowProperties": [], "typeOfFlow": "Other flow", "classification": {"classHierarchy": "Quantities / Environmental quantities / EPD EN 15804 / LCI indicators", "name": "GaBiCategories"}}, {"dataSetInternalID": 11, "referenceToFlowDataSet": {"shortDescription": [{"value": "Hazardous waste disposed (HWD)", "lang": "en"}, {"value": "Gefährlicher Abfall zur Deponie (HWD)", "lang": "de"}], "type": "flow data set", "refObjectId": "430f9e0f-59b2-46a0-8e0d-55e0e84948fc", "uri": "../flows/430f9e0f-59b2-46a0-8e0d-55e0e84948fc.xml"}, "exchange direction": "OUTPUT", "other": {"anies": [{"name": "referenceToUnitGroupDataSet", "value": {"shortDescription": [{"value": "kg", "lang": "en"}], "type": "unit group data set", "refObjectId": "ad38d542-3fe9-439d-9b95-2f5f7752acaf", "uri": "../unitgroups/ad38d542-3fe9-439d-9b95-2f5f7752acaf.xml"}}, {"value": "3.218715E-05", "module": "A1-A3"}, {"value": "3.528E-09", "module": "A4"}, {"value": "3.579E-09", "module": "A5"}, {"value": "0", "module": "B2"}, {"value": "4.074E-06", "module": "B6"}, {"value": "0", "module": "C1"}, {"value": "1.763E-09", "module": "C2"}, {"value": "1.688E-08", "module": "C3"}, {"value": "1.541E-07", "module": "C4"}, {"value": "-1.588E-06", "module": "D"}]}, "resolvedFlowVersion": "38.00.000", "flowProperties": [], "typeOfFlow": "Other flow", "classification": {"classHierarchy": "Quantities / Environmental quantities / EPD EN 15804 / LCI indicators", "name": "GaBiCategories"}}, {"dataSetInternalID": 12, "referenceToFlowDataSet": {"shortDescription": [{"value": "Non hazardous waste disposed (NHWD)", "lang": "en"}, {"value": "Entsorgter nicht gefährlicher Abfall (NHWD)", "lang": "de"}], "type": "flow data set", "refObjectId": "b29ef66b-e286-4afa-949f-62f1a7b4d7fa", "uri": "../flows/b29ef66b-e286-4afa-949f-62f1a7b4d7fa.xml"}, "exchange direction": "OUTPUT", "other": {"anies": [{"name": "referenceToUnitGroupDataSet", "value": {"shortDescription": [{"value": "kg", "lang": "en"}], "type": "unit group data set", "refObjectId": "ad38d542-3fe9-439d-9b95-2f5f7752acaf", "uri": "../unitgroups/ad38d542-3fe9-439d-9b95-2f5f7752acaf.xml"}}, {"value": "62.997", "module": "A1-A3"}, {"value": "0.004", "module": "A4"}, {"value": "0.216", "module": "A5"}, {"value": "0", "module": "B2"}, {"value": "6.983", "module": "B6"}, {"value": "0", "module": "C1"}, {"value": "0.002", "module": "C2"}, {"value": "0.989", "module": "C3"}, {"value": "50.84", "module": "C4"}, {"value": "-35.252", "module": "D"}]}, "resolvedFlowVersion": "38.00.000", "flowProperties": [], "typeOfFlow": "Other flow", "classification": {"classHierarchy": "Quantities / Environmental quantities / EPD EN 15804 / LCI indicators", "name": "GaBiCategories"}}, {"dataSetInternalID": 13, "referenceToFlowDataSet": {"shortDescription": [{"value": "Radioactive waste disposed (RWD)", "lang": "en"}, {"value": "Entsorgter radioaktiver Abfall (RWD)", "lang": "de"}], "type": "flow data set", "refObjectId": "3449546e-52ad-4b39-b809-9fb77cea8ff6", "uri": "../flows/3449546e-52ad-4b39-b809-9fb77cea8ff6.xml"}, "exchange direction": "OUTPUT", "other": {"anies": [{"name": "referenceToUnitGroupDataSet", "value": {"shortDescription": [{"value": "kg", "lang": "en"}], "type": "unit group data set", "refObjectId": "ad38d542-3fe9-439d-9b95-2f5f7752acaf", "uri": "../unitgroups/ad38d542-3fe9-439d-9b95-2f5f7752acaf.xml"}}, {"value": "0.3011456", "module": "A1-A3"}, {"value": "3.904E-05", "module": "A4"}, {"value": "5.195E-05", "module": "A5"}, {"value": "0", "module": "B2"}, {"value": "1.494", "module": "B6"}, {"value": "0", "module": "C1"}, {"value": "1.951E-05", "module": "C2"}, {"value": "0.0001863", "module": "C3"}, {"value": "0.0001151", "module": "C4"}, {"value": "-0.087", "module": "D"}]}, "resolvedFlowVersion": "38.00.000", "flowProperties": [], "typeOfFlow": "Other flow", "classification": {"classHierarchy": "Quantities / Environmental quantities / EPD EN 15804 / LCI indicators", "name": "GaBiCategories"}}, {"dataSetInternalID": 14, "referenceToFlowDataSet": {"shortDescription": [{"value": "Components for re-use (CRU)", "lang": "en"}, {"value": "Komponenten für die Wiederverwendung (CRU)", "lang": "de"}], "type": "flow data set", "refObjectId": "a2b32f97-3fc7-4af2-b209-525bc6426f33", "uri": "../flows/a2b32f97-3fc7-4af2-b209-525bc6426f33.xml"}, "exchange direction": "OUTPUT", "other": {"anies": [{"name": "referenceToUnitGroupDataSet", "value": {"shortDescription": [{"value": "kg", "lang": "en"}], "type": "unit group data set", "refObjectId": "ad38d542-3fe9-439d-9b95-2f5f7752acaf", "uri": "../unitgroups/ad38d542-3fe9-439d-9b95-2f5f7752acaf.xml"}}, {"value": "0", "module": "A1-A3"}, {"value": "0", "module": "A4"}, {"value": "0", "module": "A5"}, {"value": "0", "module": "B2"}, {"value": "0", "module": "B6"}, {"value": "0", "module": "C1"}, {"value": "0", "module": "C2"}, {"value": "0", "module": "C3"}, {"value": "0", "module": "C4"}, {"value": "0", "module": "D"}]}, "resolvedFlowVersion": "38.00.000", "flowProperties": [], "typeOfFlow": "Other flow", "classification": {"classHierarchy": "Quantities / Environmental quantities / EPD EN 15804 / LCI indicators", "name": "GaBiCategories"}}, {"dataSetInternalID": 15, "referenceToFlowDataSet": {"shortDescription": [{"value": "Materials for recycling (MFR)", "lang": "en"}, {"value": "Stoffe zum Recycling (MFR)", "lang": "de"}], "type": "flow data set", "refObjectId": "d7fe48a5-4103-49c8-9aae-b0b5dfdbd6ae", "uri": "../flows/d7fe48a5-4103-49c8-9aae-b0b5dfdbd6ae.xml"}, "exchange direction": "OUTPUT", "other": {"anies": [{"name": "referenceToUnitGroupDataSet", "value": {"shortDescription": [{"value": "kg", "lang": "en"}], "type": "unit group data set", "refObjectId": "ad38d542-3fe9-439d-9b95-2f5f7752acaf", "uri": "../unitgroups/ad38d542-3fe9-439d-9b95-2f5f7752acaf.xml"}}, {"value": "0", "module": "A1-A3"}, {"value": "0", "module": "A4"}, {"value": "0", "module": "A5"}, {"value": "0", "module": "B2"}, {"value": "0", "module": "B6"}, {"value": "0", "module": "C1"}, {"value": "0", "module": "C2"}, {"value": "250.7", "module": "C3"}, {"value": "0", "module": "C4"}, {"value": "0", "module": "D"}]}, "resolvedFlowVersion": "38.00.000", "flowProperties": [], "typeOfFlow": "Other flow", "classification": {"classHierarchy": "Quantities / Environmental quantities / EPD EN 15804 / LCI indicators", "name": "GaBiCategories"}}, {"dataSetInternalID": 16, "referenceToFlowDataSet": {"shortDescription": [{"value": "Materials for energy recovery (MER)", "lang": "en"}, {"value": "Stoffe für die Energierückgewinnung (MER)", "lang": "de"}], "type": "flow data set", "refObjectId": "59a9181c-3aaf-46ee-8b13-2b3723b6e447", "uri": "../flows/59a9181c-3aaf-46ee-8b13-2b3723b6e447.xml"}, "exchange direction": "OUTPUT", "other": {"anies": [{"name": "referenceToUnitGroupDataSet", "value": {"shortDescription": [{"value": "kg", "lang": "en"}], "type": "unit group data set", "refObjectId": "ad38d542-3fe9-439d-9b95-2f5f7752acaf", "uri": "../unitgroups/ad38d542-3fe9-439d-9b95-2f5f7752acaf.xml"}}, {"value": "0", "module": "A1-A3"}, {"value": "0", "module": "A4"}, {"value": "0", "module": "A5"}, {"value": "0", "module": "B2"}, {"value": "0", "module": "B6"}, {"value": "0", "module": "C1"}, {"value": "0", "module": "C2"}, {"value": "0", "module": "C3"}, {"value": "0", "module": "C4"}, {"value": "0", "module": "D"}]}, "resolvedFlowVersion": "38.00.000", "flowProperties": [], "typeOfFlow": "Other flow", "classification": {"classHierarchy": "Quantities / Environmental quantities / EPD EN 15804 / LCI indicators", "name": "GaBiCategories"}}, {"dataSetInternalID": 17, "referenceToFlowDataSet": {"shortDescription": [{"value": "Exported electrical energy (EEE)", "lang": "en"}, {"value": "Exportierte elektrische Energie (EEE)", "lang": "de"}], "type": "flow data set", "refObjectId": "4da0c987-2b76-40d6-9e9e-82a017aaaf29", "uri": "../flows/4da0c987-2b76-40d6-9e9e-82a017aaaf29.xml"}, "exchange direction": "OUTPUT", "other": {"anies": [{"name": "referenceToUnitGroupDataSet", "value": {"shortDescription": [{"value": "MJ", "lang": "en"}], "type": "unit group data set", "refObjectId": "93a60a57-a3c8-11da-a746-0800200c9a66", "uri": "../unitgroups/93a60a57-a3c8-11da-a746-0800200c9a66.xml"}}, {"value": "0", "module": "A1-A3"}, {"value": "0", "module": "A4"}, {"value": "5.205", "module": "A5"}, {"value": "0", "module": "B2"}, {"value": "0", "module": "B6"}, {"value": "0", "module": "C1"}, {"value": "0", "module": "C2"}, {"value": "0", "module": "C3"}, {"value": "0", "module": "C4"}, {"value": "0", "module": "D"}]}, "resolvedFlowVersion": "38.00.000", "flowProperties": [], "typeOfFlow": "Other flow", "classification": {"classHierarchy": "Quantities / Environmental quantities / EPD EN 15804 / LCI indicators", "name": "GaBiCategories"}}, {"dataSetInternalID": 18, "referenceToFlowDataSet": {"shortDescription": [{"value": "Exported thermal energy (EET)", "lang": "en"}, {"value": "Exportierte thermische Energie (EET)", "lang": "de"}], "type": "flow data set", "refObjectId": "98daf38a-7a79-46d3-9a37-2b7bd0955810", "uri": "../flows/98daf38a-7a79-46d3-9a37-2b7bd0955810.xml"}, "exchange direction": "OUTPUT", "other": {"anies": [{"name": "referenceToUnitGroupDataSet", "value": {"shortDescription": [{"value": "MJ", "lang": "en"}], "type": "unit group data set", "refObjectId": "93a60a57-a3c8-11da-a746-0800200c9a66", "uri": "../unitgroups/93a60a57-a3c8-11da-a746-0800200c9a66.xml"}}, {"value": "0", "module": "A1-A3"}, {"value": "0", "module": "A4"}, {"value": "10.915", "module": "A5"}, {"value": "0", "module": "B2"}, {"value": "0", "module": "B6"}, {"value": "0", "module": "C1"}, {"value": "0", "module": "C2"}, {"value": "0", "module": "C3"}, {"value": "0", "module": "C4"}, {"value": "0", "module": "D"}]}, "resolvedFlowVersion": "38.00.000", "flowProperties": [], "typeOfFlow": "Other flow", "classification": {"classHierarchy": "Quantities / Environmental quantities / EPD EN 15804 / LCI indicators", "name": "GaBiCategories"}}]}, "LCIAResults": {"LCIAResult": [{"referenceToLCIAMethodDataSet": {"shortDescription": [{"value": "Global Warming Potential total (GWP-total)", "lang": "en"}, {"value": "Globales Erwärmungspotenzial total (GWP-total)", "lang": "de"}], "type": "LCIA method data set", "refObjectId": "6a37f984-a4b3-458a-a20a-64418c145fa2", "uri": "../lciamethods/6a37f984-a4b3-458a-a20a-64418c145fa2.xml"}, "other": {"anies": [{"name": "referenceToUnitGroupDataSet", "value": {"shortDescription": [{"value": "kg CO_(2) eq", "lang": "en"}], "type": "unit group data set", "refObjectId": "1ebf3012-d0db-4de2-aefd-ef30cedb0be1", "uri": "../unitgroups/1ebf3012-d0db-4de2-aefd-ef30cedb0be1.xml"}}, {"value": "678.955", "module": "A1-A3"}, {"value": "2.681", "module": "A4"}, {"value": "3.07", "module": "A5"}, {"value": "0", "module": "B2"}, {"value": "562.49", "module": "B6"}, {"value": "0", "module": "C1"}, {"value": "1.34", "module": "C2"}, {"value": "11.404", "module": "C3"}, {"value": "0.775", "module": "C4"}, {"value": "-290.4", "module": "D"}]}}, {"referenceToLCIAMethodDataSet": {"shortDescription": [{"value": "Global Warming Potential fossil fuels (GWP-fossil)", "lang": "en"}, {"value": "Globales Erwärmungspotenzial fossil (GWP-fossil)", "lang": "de"}], "type": "LCIA method data set", "refObjectId": "5f635281-343e-44fb-83df-1971b155e6b6", "uri": "../lciamethods/5f635281-343e-44fb-83df-1971b155e6b6.xml"}, "other": {"anies": [{"name": "referenceToUnitGroupDataSet", "value": {"shortDescription": [{"value": "kg CO_(2) eq", "lang": "en"}], "type": "unit group data set", "refObjectId": "1ebf3012-d0db-4de2-aefd-ef30cedb0be1", "uri": "../unitgroups/1ebf3012-d0db-4de2-aefd-ef30cedb0be1.xml"}}, {"value": "681.343", "module": "A1-A3"}, {"value": "2.562", "module": "A4"}, {"value": "1.688", "module": "A5"}, {"value": "0", "module": "B2"}, {"value": "559.81", "module": "B6"}, {"value": "0", "module": "C1"}, {"value": "1.28", "module": "C2"}, {"value": "9.414", "module": "C3"}, {"value": "0.77", "module": "C4"}, {"value": "-291.02", "module": "D"}]}}, {"referenceToLCIAMethodDataSet": {"shortDescription": [{"value": "Global Warming Potential biogenic (GWP-biogenic)", "lang": "en"}, {"value": "Globales Erwärmungspotenzial biogen (GWP-biogenic)", "lang": "de"}], "type": "LCIA method data set", "refObjectId": "2356e1ab-0185-4db5-86e5-16de51c7485c", "uri": "../lciamethods/2356e1ab-0185-4db5-86e5-16de51c7485c.xml"}, "other": {"anies": [{"name": "referenceToUnitGroupDataSet", "value": {"shortDescription": [{"value": "kg CO_(2) eq", "lang": "en"}], "type": "unit group data set", "refObjectId": "1ebf3012-d0db-4de2-aefd-ef30cedb0be1", "uri": "../unitgroups/1ebf3012-d0db-4de2-aefd-ef30cedb0be1.xml"}}, {"value": "-3.446", "module": "A1-A3"}, {"value": "0.118", "module": "A4"}, {"value": "1.382", "module": "A5"}, {"value": "0", "module": "B2"}, {"value": "1.866", "module": "B6"}, {"value": "0", "module": "C1"}, {"value": "0.059", "module": "C2"}, {"value": "1.99", "module": "C3"}, {"value": "0.003", "module": "C4"}, {"value": "1.114", "module": "D"}]}}, {"referenceToLCIAMethodDataSet": {"shortDescription": [{"value": "Global Warming Potential luluc (GWP-luluc)", "lang": "en"}, {"value": "Globales Erwärmungspotenzial luluc (GWP-luluc)", "lang": "de"}], "type": "LCIA method data set", "refObjectId": "4331bbdb-978a-490d-8707-eeb047f01a55", "uri": "../lciamethods/4331bbdb-978a-490d-8707-eeb047f01a55.xml"}, "other": {"anies": [{"name": "referenceToUnitGroupDataSet", "value": {"shortDescription": [{"value": "kg CO_(2) eq", "lang": "en"}], "type": "unit group data set", "refObjectId": "1ebf3012-d0db-4de2-aefd-ef30cedb0be1", "uri": "../unitgroups/1ebf3012-d0db-4de2-aefd-ef30cedb0be1.xml"}}, {"value": "1.0592274", "module": "A1-A3"}, {"value": "6.098E-05", "module": "A4"}, {"value": "0.0001167", "module": "A5"}, {"value": "0", "module": "B2"}, {"value": "0.811", "module": "B6"}, {"value": "0", "module": "C1"}, {"value": "3.047E-05", "module": "C2"}, {"value": "0.0005499", "module": "C3"}, {"value": "0.002", "module": "C4"}, {"value": "-0.495", "module": "D"}]}}, {"referenceToLCIAMethodDataSet": {"shortDescription": [{"value": "Depletion potential of the stratospheric ozone layer (ODP)", "lang": "en"}, {"value": "Abbau Potential der stratosphärischen Ozonschicht (ODP)", "lang": "de"}], "type": "LCIA method data set", "refObjectId": "b5c629d6-def3-11e6-bf01-fe55135034f3", "uri": "../lciamethods/b5c629d6-def3-11e6-bf01-fe55135034f3.xml"}, "other": {"anies": [{"name": "referenceToUnitGroupDataSet", "value": {"shortDescription": [{"value": "kg CFC11 eq", "lang": "en"}], "type": "unit group data set", "refObjectId": "d9e957c9-7309-4474-bf3a-7777df6c4e5b", "uri": "../unitgroups/d9e957c9-7309-4474-bf3a-7777df6c4e5b.xml"}}, {"value": "2.86581009E-10", "module": "A1-A3"}, {"value": "2.705E-16", "module": "A4"}, {"value": "1.089E-15", "module": "A5"}, {"value": "0", "module": "B2"}, {"value": "1.231E-11", "module": "B6"}, {"value": "0", "module": "C1"}, {"value": "1.352E-16", "module": "C2"}, {"value": "4.978E-15", "module": "C3"}, {"value": "2.857E-15", "module": "C4"}, {"value": "-3.336E-10", "module": "D"}]}}, {"referenceToLCIAMethodDataSet": {"shortDescription": [{"value": "Acidification potential of land and water (AP)", "lang": "en"}, {"value": "Versauerungspotenzial von Boden und Wasser (AP)", "lang": "de"}], "type": "LCIA method data set", "refObjectId": "b5c611c6-def3-11e6-bf01-fe55135034f3", "uri": "../lciamethods/b5c611c6-def3-11e6-bf01-fe55135034f3.xml"}, "other": {"anies": [{"name": "referenceToUnitGroupDataSet", "value": {"shortDescription": [{"value": "mol H^(+) eq", "lang": "en"}], "type": "unit group data set", "refObjectId": "42e089ac-92bf-4bf2-8ca1-5fc40d18f2ed", "uri": "../unitgroups/42e089ac-92bf-4bf2-8ca1-5fc40d18f2ed.xml"}}, {"value": "3.093", "module": "A1-A3"}, {"value": "0.003", "module": "A4"}, {"value": "0.0006912", "module": "A5"}, {"value": "0", "module": "B2"}, {"value": "1.236", "module": "B6"}, {"value": "0", "module": "C1"}, {"value": "0.001", "module": "C2"}, {"value": "0.002", "module": "C3"}, {"value": "0.006", "module": "C4"}, {"value": "-1.284", "module": "D"}]}}, {"referenceToLCIAMethodDataSet": {"shortDescription": [{"value": "Eutrophication potential aquatic freshwater (EP-freshwater)", "lang": "en"}, {"value": "Eutrophierungspotenzial Süßwasser (EP-freshwater)", "lang": "de"}], "type": "LCIA method data set", "refObjectId": "b53ec18f-7377-4ad3-86eb-cc3f4f276b2b", "uri": "../lciamethods/b53ec18f-7377-4ad3-86eb-cc3f4f276b2b.xml"}, "other": {"anies": [{"name": "referenceToUnitGroupDataSet", "value": {"shortDescription": [{"value": "kg P eq", "lang": "en"}], "type": "unit group data set", "refObjectId": "0429039d-a61d-4590-ba67-aa4a20a810a1", "uri": "../unitgroups/0429039d-a61d-4590-ba67-aa4a20a810a1.xml"}}, {"value": "0.001157545", "module": "A1-A3"}, {"value": "5.484E-07", "module": "A4"}, {"value": "1.829E-07", "module": "A5"}, {"value": "0", "module": "B2"}, {"value": "0.001", "module": "B6"}, {"value": "0", "module": "C1"}, {"value": "2.74E-07", "module": "C2"}, {"value": "7.914E-07", "module": "C3"}, {"value": "1.323E-06", "module": "C4"}, {"value": "-0.0002402", "module": "D"}]}}, {"referenceToLCIAMethodDataSet": {"shortDescription": [{"value": "Eutrophication potential aquatic marine (EP-marine)", "lang": "en"}, {"value": "Eutrophierungspotenzial Salzwasser (EP-marine)", "lang": "de"}], "type": "LCIA method data set", "refObjectId": "b5c619fa-def3-11e6-bf01-fe55135034f3", "uri": "../lciamethods/b5c619fa-def3-11e6-bf01-fe55135034f3.xml"}, "other": {"anies": [{"name": "referenceToUnitGroupDataSet", "value": {"shortDescription": [{"value": "kg N eq", "lang": "en"}], "type": "unit group data set", "refObjectId": "d05bb823-ecdf-4686-8c40-bf1d9257859f", "uri": "../unitgroups/d05bb823-ecdf-4686-8c40-bf1d9257859f.xml"}}, {"value": "0.443", "module": "A1-A3"}, {"value": "0.000816", "module": "A4"}, {"value": "0.0002097", "module": "A5"}, {"value": "0", "module": "B2"}, {"value": "0.275", "module": "B6"}, {"value": "0", "module": "C1"}, {"value": "0.0004077", "module": "C2"}, {"value": "0.0004707", "module": "C3"}, {"value": "0.001", "module": "C4"}, {"value": "-0.195", "module": "D"}]}}, {"referenceToLCIAMethodDataSet": {"shortDescription": [{"value": "Eutrophication potential terrestrial (EP-terrestrial)", "lang": "en"}, {"value": "Eutrophierungspotenzial Land (EP-terrestrial)", "lang": "de"}], "type": "LCIA method data set", "refObjectId": "b5c614d2-def3-11e6-bf01-fe55135034f3", "uri": "../lciamethods/b5c614d2-def3-11e6-bf01-fe55135034f3.xml"}, "other": {"anies": [{"name": "referenceToUnitGroupDataSet", "value": {"shortDescription": [{"value": "mol N eq", "lang": "en"}], "type": "unit group data set", "refObjectId": "71b4d617-0ec9-4d3f-b65e-e438940c2401", "uri": "../unitgroups/71b4d617-0ec9-4d3f-b65e-e438940c2401.xml"}}, {"value": "4.792", "module": "A1-A3"}, {"value": "0.009", "module": "A4"}, {"value": "0.003", "module": "A5"}, {"value": "0", "module": "B2"}, {"value": "2.884", "module": "B6"}, {"value": "0", "module": "C1"}, {"value": "0.005", "module": "C2"}, {"value": "0.009", "module": "C3"}, {"value": "0.016", "module": "C4"}, {"value": "-2.123", "module": "D"}]}}, {"referenceToLCIAMethodDataSet": {"shortDescription": [{"value": "Formation potential of tropospheric ozone photochemical oxidants (POCP)", "lang": "en"}, {"value": "Bildungspotential für troposphärisches Ozon (POCP)", "lang": "de"}], "type": "LCIA method data set", "refObjectId": "b5c610fe-def3-11e6-bf01-fe55135034f3", "uri": "../lciamethods/b5c610fe-def3-11e6-bf01-fe55135034f3.xml"}, "other": {"anies": [{"name": "referenceToUnitGroupDataSet", "value": {"shortDescription": [{"value": "kg NMVOC eq", "lang": "en"}], "type": "unit group data set", "refObjectId": "d27c25f8-fbc1-44c6-b47b-4adbae4199c6", "uri": "../unitgroups/d27c25f8-fbc1-44c6-b47b-4adbae4199c6.xml"}}, {"value": "1.375", "module": "A1-A3"}, {"value": "0.002", "module": "A4"}, {"value": "0.0005636", "module": "A5"}, {"value": "0", "module": "B2"}, {"value": "0.752", "module": "B6"}, {"value": "0", "module": "C1"}, {"value": "0.001", "module": "C2"}, {"value": "0.001", "module": "C3"}, {"value": "0.004", "module": "C4"}, {"value": "-0.582", "module": "D"}]}}, {"referenceToLCIAMethodDataSet": {"shortDescription": [{"value": "Abiotic depletion potential for non fossil resources (ADPE)", "lang": "en"}, {"value": "Potenzial für den abiotischen Abbau nicht fossiler Ressourcen (ADPE)", "lang": "de"}], "type": "LCIA method data set", "refObjectId": "b2ad6494-c78d-11e6-9d9d-cec0c932ce01", "uri": "../lciamethods/b2ad6494-c78d-11e6-9d9d-cec0c932ce01.xml"}, "other": {"anies": [{"name": "referenceToUnitGroupDataSet", "value": {"shortDescription": [{"value": "kg Sb eq", "lang": "en"}], "type": "unit group data set", "refObjectId": "54ccd2d9-a32a-4fc2-923d-f2c8c93e89d4", "uri": "../unitgroups/54ccd2d9-a32a-4fc2-923d-f2c8c93e89d4.xml"}}, {"value": "0.0310002865", "module": "A1-A3"}, {"value": "7.684E-08", "module": "A4"}, {"value": "1.546E-08", "module": "A5"}, {"value": "0", "module": "B2"}, {"value": "0.000162", "module": "B6"}, {"value": "0", "module": "C1"}, {"value": "3.84E-08", "module": "C2"}, {"value": "6.882E-08", "module": "C3"}, {"value": "6.92E-08", "module": "C4"}, {"value": "-0.008", "module": "D"}]}}, {"referenceToLCIAMethodDataSet": {"shortDescription": [{"value": "Abiotic depletion potential for fossil resources (ADPF)", "lang": "en"}, {"value": "Potenzial für den abiotischen Abbau fossiler Brennstoffe (ADPF)", "lang": "de"}], "type": "LCIA method data set", "refObjectId": "b2ad6110-c78d-11e6-9d9d-cec0c932ce01", "uri": "../lciamethods/b2ad6110-c78d-11e6-9d9d-cec0c932ce01.xml"}, "other": {"anies": [{"name": "referenceToUnitGroupDataSet", "value": {"shortDescription": [{"value": "MJ", "lang": "en"}], "type": "unit group data set", "refObjectId": "93a60a57-a3c8-11da-a746-0800200c9a66", "uri": "../unitgroups/93a60a57-a3c8-11da-a746-0800200c9a66.xml"}}, {"value": "8829.97", "module": "A1-A3"}, {"value": "36.333", "module": "A4"}, {"value": "1.213", "module": "A5"}, {"value": "0", "module": "B2"}, {"value": "9841.2", "module": "B6"}, {"value": "0", "module": "C1"}, {"value": "18.155", "module": "C2"}, {"value": "4.784", "module": "C3"}, {"value": "10.108", "module": "C4"}, {"value": "-3655", "module": "D"}]}}, {"referenceToLCIAMethodDataSet": {"shortDescription": [{"value": "Water use (WDP)", "lang": "en"}, {"value": "Wassernutzung (WDP)", "lang": "de"}], "type": "LCIA method data set", "refObjectId": "b2ad66ce-c78d-11e6-9d9d-cec0c932ce01", "uri": "../lciamethods/b2ad66ce-c78d-11e6-9d9d-cec0c932ce01.xml"}, "other": {"anies": [{"name": "referenceToUnitGroupDataSet", "value": {"shortDescription": [{"value": "m^(3) world eq deprived", "lang": "en"}], "type": "unit group data set", "refObjectId": "6ae2df01-888e-46c8-b17d-49fa3869b476", "uri": "../unitgroups/6ae2df01-888e-46c8-b17d-49fa3869b476.xml"}}, {"value": "194.629", "module": "A1-A3"}, {"value": "0.005", "module": "A4"}, {"value": "0.345", "module": "A5"}, {"value": "0", "module": "B2"}, {"value": "122.02", "module": "B6"}, {"value": "0", "module": "C1"}, {"value": "0.003", "module": "C2"}, {"value": "1.168", "module": "C3"}, {"value": "0.081", "module": "C4"}, {"value": "-103.4", "module": "D"}]}}, {"referenceToLCIAMethodDataSet": {"shortDescription": [{"value": "Incidence of disease due to PM emissions (PM)", "lang": "en"}, {"value": "Auftreten von Krankheiten aufgrund von Feinstaubemissionen (PM)", "lang": "de"}], "type": "LCIA method data set", "refObjectId": "b5c602c6-def3-11e6-bf01-fe55135034f3", "uri": "../lciamethods/b5c602c6-def3-11e6-bf01-fe55135034f3.xml"}, "other": {"anies": [{"name": "referenceToUnitGroupDataSet", "value": {"shortDescription": [{"value": "Disease incidence", "lang": "en"}], "type": "unit group data set", "refObjectId": "3883559b-648f-4afc-8ba2-0bd24f3affa3", "uri": "../unitgroups/3883559b-648f-4afc-8ba2-0bd24f3affa3.xml"}}, {"value": "4.852724E-05", "module": "A1-A3"}, {"value": "1.348E-08", "module": "A4"}, {"value": "5.953E-09", "module": "A5"}, {"value": "0", "module": "B2"}, {"value": "1.037E-05", "module": "B6"}, {"value": "0", "module": "C1"}, {"value": "6.736E-09", "module": "C2"}, {"value": "2.277E-08", "module": "C3"}, {"value": "6.842E-08", "module": "C4"}, {"value": "-2.498E-05", "module": "D"}]}}, {"referenceToLCIAMethodDataSet": {"shortDescription": [{"value": "Human exposure efficiency relative to U235 (IR)", "lang": "en"}, {"value": "Wirkung durch Exposition des Menschen mit U235 (IR)", "lang": "de"}], "type": "LCIA method data set", "refObjectId": "b5c632be-def3-11e6-bf01-fe55135034f3", "uri": "../lciamethods/b5c632be-def3-11e6-bf01-fe55135034f3.xml"}, "other": {"anies": [{"name": "referenceToUnitGroupDataSet", "value": {"shortDescription": [{"value": "kBq U235 eq", "lang": "en"}], "type": "unit group data set", "refObjectId": "456b05bf-1415-44a9-9993-02452f554c09", "uri": "../unitgroups/456b05bf-1415-44a9-9993-02452f554c09.xml"}}, {"value": "40.096", "module": "A1-A3"}, {"value": "0.006", "module": "A4"}, {"value": "0.006", "module": "A5"}, {"value": "0", "module": "B2"}, {"value": "245.05", "module": "B6"}, {"value": "0", "module": "C1"}, {"value": "0.003", "module": "C2"}, {"value": "0.018", "module": "C3"}, {"value": "0.012", "module": "C4"}, {"value": "-16.285", "module": "D"}]}}, {"referenceToLCIAMethodDataSet": {"shortDescription": [{"value": "Comparative toxic unit for ecosystems (ETP-fw)", "lang": "en"}, {"value": "Toxizitätsvergleichseinheit für Ökosysteme (ETP-fw)", "lang": "de"}], "type": "LCIA method data set", "refObjectId": "ee1082d1-b0f7-43ca-a1f0-21e2a4a74511", "uri": "../lciamethods/ee1082d1-b0f7-43ca-a1f0-21e2a4a74511.xml"}, "other": {"anies": [{"name": "referenceToUnitGroupDataSet", "value": {"shortDescription": [{"value": "CTUe", "lang": "en"}], "type": "unit group data set", "refObjectId": "aa959ded-f1eb-4efb-9c5c-2d60be36b3e6", "uri": "../unitgroups/aa959ded-f1eb-4efb-9c5c-2d60be36b3e6.xml"}}, {"value": "3811.594", "module": "A1-A3"}, {"value": "25.756", "module": "A4"}, {"value": "0.5", "module": "A5"}, {"value": "0", "module": "B2"}, {"value": "4209.9", "module": "B6"}, {"value": "0", "module": "C1"}, {"value": "12.869", "module": "C2"}, {"value": "1.822", "module": "C3"}, {"value": "5.776", "module": "C4"}, {"value": "-1829.8", "module": "D"}]}}, {"referenceToLCIAMethodDataSet": {"shortDescription": [{"value": "Comparative toxic unit for humans (carcinogenic) (HTP-c)", "lang": "en"}, {"value": "Toxizitätsvergleichseinheit für Menschen (krebserregend) (HTP-c)", "lang": "de"}], "type": "LCIA method data set", "refObjectId": "2299222a-bbd8-474f-9d4f-4dd1f18aea7c", "uri": "../lciamethods/2299222a-bbd8-474f-9d4f-4dd1f18aea7c.xml"}, "other": {"anies": [{"name": "referenceToUnitGroupDataSet", "value": {"shortDescription": [{"value": "CTUh", "lang": "en"}], "type": "unit group data set", "refObjectId": "d4c9523e-2d7e-49fd-8469-998f547d3a70", "uri": "../unitgroups/d4c9523e-2d7e-49fd-8469-998f547d3a70.xml"}}, {"value": "7.9686976E-05", "module": "A1-A3"}, {"value": "4.844E-10", "module": "A4"}, {"value": "3.612E-11", "module": "A5"}, {"value": "0", "module": "B2"}, {"value": "1.163E-07", "module": "B6"}, {"value": "0", "module": "C1"}, {"value": "2.421E-10", "module": "C2"}, {"value": "1.539E-10", "module": "C3"}, {"value": "8.558E-10", "module": "C4"}, {"value": "-5.268E-07", "module": "D"}]}}, {"referenceToLCIAMethodDataSet": {"shortDescription": [{"value": "Comparative toxic unit for humans (noncarcinogenic) (HTP-nc)", "lang": "en"}, {"value": "Toxizitätsvergleichseinheit für Menschen (nicht krebserregend) (HTP-nc)", "lang": "de"}], "type": "LCIA method data set", "refObjectId": "3af763a5-b7a1-48c9-9cee-1f223481fcef", "uri": "../lciamethods/3af763a5-b7a1-48c9-9cee-1f223481fcef.xml"}, "other": {"anies": [{"name": "referenceToUnitGroupDataSet", "value": {"shortDescription": [{"value": "CTUh", "lang": "en"}], "type": "unit group data set", "refObjectId": "d4c9523e-2d7e-49fd-8469-998f547d3a70", "uri": "../unitgroups/d4c9523e-2d7e-49fd-8469-998f547d3a70.xml"}}, {"value": "1.233105E-05", "module": "A1-A3"}, {"value": "2.072E-08", "module": "A4"}, {"value": "3.006E-09", "module": "A5"}, {"value": "0", "module": "B2"}, {"value": "4.284E-06", "module": "B6"}, {"value": "0", "module": "C1"}, {"value": "1.035E-08", "module": "C2"}, {"value": "1.475E-08", "module": "C3"}, {"value": "9.433E-08", "module": "C4"}, {"value": "-1.556E-06", "module": "D"}]}}, {"referenceToLCIAMethodDataSet": {"shortDescription": [{"value": "Soil quality index (SQP)", "lang": "en"}, {"value": "Bodenqualitätsindex (SQP)", "lang": "de"}], "type": "LCIA method data set", "refObjectId": "b2ad6890-c78d-11e6-9d9d-cec0c932ce01", "uri": "../lciamethods/b2ad6890-c78d-11e6-9d9d-cec0c932ce01.xml"}, "other": {"anies": [{"name": "referenceToUnitGroupDataSet", "value": {"shortDescription": [{"value": "SQP", "lang": "en"}], "type": "unit group data set", "refObjectId": "f130951c-e67f-4f7f-8dd4-665de3974e18", "uri": "../unitgroups/f130951c-e67f-4f7f-8dd4-665de3974e18.xml"}}, {"value": "2132.258", "module": "A1-A3"}, {"value": "0.093", "module": "A4"}, {"value": "0.348", "module": "A5"}, {"value": "0", "module": "B2"}, {"value": "3134.4", "module": "B6"}, {"value": "0", "module": "C1"}, {"value": "0.047", "module": "C2"}, {"value": "1.423", "module": "C3"}, {"value": "2.107", "module": "C4"}, {"value": "-465.87", "module": "D"}]}}]}, "otherAttributes": {"{http://www.indata.network/EPD/2019}epd-version": "1.2"}, "version": "1.1", "locations": "../ILCDLocations.xml"}