{"processInformation": {"dataSetInformation": {"UUID": "d654ea26-a0aa-4361-b01e-9281038f6a27", "name": {"baseName": [{"value": "Fibrolith® mineralisch gebundene Holzwolleplatten (Monoplatten der Baustoffklasse A2)", "lang": "de"}, {"value": "Fibrolith® mineral-bonded wood wool panels (mono-panels of building materials class A2)", "lang": "en"}], "functionalUnitFlowProperties": [{"lang": "de"}]}, "classificationInformation": {"classification": [{"class": [{"value": "Dämmstoffe", "level": 0, "classId": "2"}, {"value": "Holzwolleplatten", "level": 1, "classId": "2.7"}, {"value": "Holzwolleleichtbauplatten", "level": 2, "classId": "2.7.01"}], "name": "OEKOBAU.DAT"}, {"class": [{"value": "02 Bauprodukte", "level": 0}, {"value": "Holzwerkstoffe", "level": 1}, {"value": "Holzzement - Mineralisch gebundene Holzwerkstoffe", "level": 2}], "name": "IBUCategories"}]}, "generalComment": [{"value": "Die deklarierten Fibro-Kustik Platten aus mineralisch gebundener Holzwolle der Baustoffklasse A2 werden unter folgenden Produktnamen vertrieben:\n\nFibro-Kustik Florence\n\nFibro-Kustik Paris\nDie Fibro-Kustik Platten werden aus Holzwolle und mineralischem Bindemittel hergestellt. Neben naturbelassener Optik knnen die Platten in allen RAL- und NCS-Tnen gespritzt werden und eine zustzliche Beschichtung mit Pure Genius erhalten, um eine raumluftreinigende Wirkung durch Photokatalyse zu erhalten.", "lang": "de"}, {"value": "The declared Fibro-Kustik panels made of mineral-bonded wood wool of building materials class A2 are distributed under the following product names:\n Fibro-Kustik Florence\n Fibro-Kustik Paris \nThe Fibro-Kustik panels are manufactured from wood wool and mineral binding agent. In addition to the natural look, the panels can be sprayed in all RAL and NCS colours and given an additional coating with Pure Genius to achieve an indoor air purifying effect through photocatalysis.", "lang": "en"}]}, "quantitativeReference": {"referenceToReferenceFlow": [0]}, "time": {"referenceYear": 2024, "dataSetValidUntil": 2029, "other": {"anies": [{"name": "publicationDateOfEPD", "value": 1707955200000}]}}, "geography": {"locationOfOperationSupplyOrProduction": {"location": "DE"}}, "technology": {"technologyDescriptionAndIncludedProcesses": [{"value": "Bereits entrindete Fichtenholzstämme mit 2m Länge werden nach ihrer Anlieferung 6 bis 12 Monate gelagert, bis ihre Restfeuchte auf 27 % gefallen ist. Anschließend werden sie mechanisch zu Holzwolle verarbeitet. Die Holzwolle wird angefeuchtet und in einem Zweiwellenmischer mit dem Portlandzement vermischt. Das entstandene Mischgut wird in Formen gestreut, mehrmals gepresst und gestapelt. Die Stapel werden mit einem Gewicht belastet und zum ersten Aushärten gelagert. Nach etwa 24 Stunden hat der Zement durch den Abbindeprozess eine ausreichende Festigkeit erreicht, damit die Platten ausgeschalt werden können. Anschließend werden die Platten nochmals mehrere Tage stehen gelassen, damit der Zement fester werden kann, um dann in einem gasbetriebenen Trockenofen die Restfeuchte zu entfernen. Abschließend werden die getrockneten Platten konfektioniert und bei Bedarf noch lackiert oder direkt zum Versand verpackt. Die deklarierten fibrolith® zementgebundene Holzwolleplatten (Monoplatten) bestehen aus: Fichtenholz: 40% - 50% Portlandzement: 24% - 52% Wasser: 8% Abbindebeschleuniger <0,1% Das Fichtenholz wird aus nachhaltiger und PEFC- bzw. FSC-zertifizierter Forstwirtschaft bezogen. Der Weißzement dient als Bindemittel, damit die Platten die notwendige Stabilität erreichen. Wasser wird größtenteils als Kristallwasser im Zement gebunden, verbleibt aber auch zu einem geringen Teil als Restfeuchte in der Platte. Der Abbindebeschleuniger reduziert die notwendige Abbindezeit des Zements. \nDeklarierte Einheit: \nDie deklarierte Einheit ist 1 t Fibrolith® mineralisch gebundene Holzwolleplatten (Monoplatten der Baustoffklasse A2).", "lang": "de"}, {"value": "Bereits entrindete Fichtenholzstämme mit 2m Länge werden nach ihrer Anlieferung 6 bis 12 Monate gelagert, bis ihre Restfeuchte auf 27 % gefallen ist. Anschließend werden sie mechanisch zu Holzwolle verarbeitet. Die Holzwolle wird angefeuchtet und in einem Zweiwellenmischer mit dem Portlandzement vermischt. Das entstandene Mischgut wird in Formen gestreut, mehrmals gepresst und gestapelt. Die Stapel werden mit einem Gewicht belastet und zum ersten Aushärten gelagert. Nach etwa 24 Stunden hat der Zement durch den Abbindeprozess eine ausreichende Festigkeit erreicht, damit die Platten ausgeschalt werden können. Anschließend werden die Platten nochmals mehrere Tage stehen gelassen, damit der Zement fester werden kann, um dann in einem gasbetriebenen Trockenofen die Restfeuchte zu entfernen. Abschließend werden die getrockneten Platten konfektioniert und bei Bedarf noch lackiert oder direkt zum Versand verpackt. Die deklarierten fibrolith® zementgebundene Holzwolleplatten (Monoplatten) bestehen aus: Fichtenholz: 40% - 50% Portlandzement: 24% - 52% Wasser: 8% Abbindebeschleuniger <0,1% Das Fichtenholz wird aus nachhaltiger und PEFC- bzw. FSC-zertifizierter Forstwirtschaft bezogen. Der Weißzement dient als Bindemittel, damit die Platten die notwendige Stabilität erreichen. Wasser wird größtenteils als Kristallwasser im Zement gebunden, verbleibt aber auch zu einem geringen Teil als Restfeuchte in der Platte. Der Abbindebeschleuniger reduziert die notwendige Abbindezeit des Zements. \nDeclared unit: \nThe declared unit is one tonne Fibrolith® mineral-bonded wood wool panels (mono-panels of building materials class A2).", "lang": "en"}], "technologicalApplicability": [{"value": "Fibro-Kustik Platten dienen als akustische und dekorative Decken- und Wandbekleidung im Wohnungs- und Nichtwohnungsbau, z.B. Gewerbe-, Industrie- und ffentlichen Gebuden, Bros, Schulen, Sporthallen, Garagen etc. nach DIN 4108-10: DI dm / WI dm.", "lang": "de"}, {"value": "Fibro-Kustik panels serve as acoustic and decorative ceiling and wall cladding in residential and non-residential buildings, e.g. commercial properties, industrial and public buildings, offices, schools, sports centres, garages etc. in accordance with DIN 4108-10: DI dm / WI dm.", "lang": "en"}]}}, "modellingAndValidation": {"LCIMethodAndAllocation": {"typeOfDataSet": "EPD", "referenceToLCAMethodDetails": [{"shortDescription": [{"value": "Holzzement - Mineralisch gebundene Holzwerkstoffe.pdf", "lang": "de"}], "type": "source data set", "refObjectId": "97f40d2d-efdc-4d6d-a9d7-224c0b3a649a"}], "other": {"anies": [{"name": "subType", "value": "specific dataset"}]}}, "dataSourcesTreatmentAndRepresentativeness": {"referenceToDataSource": [{"shortDescription": [{"value": "ecoinvent database (all versions)", "lang": "de"}], "type": "source data set", "refObjectId": "b497a91f-e14b-4b69-8f28-f50eb1576766"}, {"shortDescription": [{"value": "ecoinvent 3.8 database", "lang": "de"}], "type": "source data set", "refObjectId": "0f4c65c0-6210-450f-b886-82bf8dd5ace9"}], "useAdviceForDataSet": [{"value": "Gültigkeitsbereich: \nDiese EPD gilt fr Fibrolith® mineralisch gebundene Holzwolleplatten (Monoplatten der Baustoffklasse A2), die im Werk der Fibrolith® Dmmstoffe GmbH in Kempenich (D) hergestellt werden. \nSystemgrenze: \nTyp der EPD: \"von der Wiege bis zum Werkstor mit Optionen, das heit, Module C1-C4 und Modul D (A1-A3, C, D und zustzliche Module. Die zustzlichen Module drfen A4 und/oder A5 und/oder B1-B7 sein)\".\n\nDer Transport auf die Baustelle (Modul A4) wird nicht modelliert und muss fallspezifisch bei einer Gebudebewertung bercksichtigt werden.\n\nFr den Einbau in Modul A5 wird von einem manuellen Einbau ausgegangen; der Stromverbrauch fr die Montage (Akkuschrauber) und Befestigungsmittel (Dbel/Schrauben) werden vernachlssigt.\n\nIn Modul A5 wird die Entsorgung der Verpackung modelliert, wobei Karton rezykliert und die Polyethylen- bzw. Holzverpackung in einer Mllverbrennungsanlage thermisch verwertet wird.\n\nWhrend der Nutzung (Modul B1) karbonatisiert das Bindemiitel in den Holzwolleplatten, womit CO2 aus der Atmosphre rckgebunden wird.\n\nGenerell knnen alle Platten nach der Demontage wieder montiert und genutzt werden. Sofern die Platten beschdigt oder nicht mehr einsetzbar sind, knnen Einschichtplatten thermisch verwertet werden.\n\nFr den Rckbau wird analog zum Einbau ein manueller Rckbau angenommen, der Stromverbrauch fr die Demontage (Akkuschrauber) wird vernachlssigt; somit sind die Werte in Modul C1 gleich null.\n\nIn Modul C2 werden die Platten zu einer Mllverbrennungsanlage transportiert.\n\nIn Modul C3 werden die Monoplatten thermisch in einer Mllverbrennungsanlage verwertet.\n\nDie Vorteile und Lasten auerhalb des Produktsystems (Modul D) umfassen die exportierte Energie aus der energetischen Verwertung der Verpackung in Modul A5 sowie aus der energetischen Verwertung der Monoplatten (Modul C3). Ersetzt wird dabei durch den exportierten Strom der Deutsche Verbrauchsmix und durch die exportierte Wrme die Wrme ab einer Gasfeuerung.", "lang": "de"}, {"value": "Scope: \nThis EPD applies for Fibrolith® mineral-bonded wood wool panels (mono-panels of building materials class A2) manufactured in the Fibrolith® Dmmstoffe GmbH plant in Kempenich (Germany). \nSystem boundary: \nType of EPD: from the cradle to the factory gate with options, i.e. modules C1-C4 and module D (A1-A3, C, D and additional modules. The additional modules may be A4 and/or A5 and/or B1-B7). \n\nTransport to the construction site (module A4) is not modelled and must be taken into account on a case-by-case basis in a building assessment. \n\nManual installation is assumed for installation in module A5; the electricity consumption for installation (cordless screwdriver) and fasteners (dowels/screws) is not taken into consideration. \n\nDisposal of the packaging is modelled in module A5, whereby cardboard is recycled and the polyethylene or wood packaging is thermally recycled in a waste incineration plant. \n\nDuring use (module B1), the binder in the wood wool panels carbonates, which absorbs CO2 from the atmosphere. \n\nIn general, all panels can be reassembled and reused after dismantling. If the panels are damaged or can no longer be used, single-layer panels can be thermally utilised. \n\nFor dismantling, manual dismantling is assumed in the same way as for installation; the electricity consumption for dismantling (cordless screwdriver) is not taken into consideration; the values in module C1 are therefore zero. \n\nThe panels are transported to a waste incineration plant in module C2. \n\nThe mono-panels are recycled thermally in a waste incineration plant in module C3. \n\nThe benefits and loads outside the product system (module D) include the exported energy from the energy recovery of the packaging in module A5 and from the energy recovery of the mono-panels (module C3). The exported electricity replaces the German consumption mix and the exported heat replaces the heat from a gas firing system.", "lang": "en"}], "other": {"anies": [{"name": "referenceToOriginalEPD", "value": {"shortDescription": {"value": "Fibrolith® mineralisch gebundene Holzwolleplatten (Monoplatten der Baustoffklasse A2).pdf", "defaultValue": "Fibrolith® mineralisch gebundene Holzwolleplatten (Monoplatten der Baustoffklasse A2).pdf", "lstrings": [{"lang": "de", "value": "Fibrolith® mineralisch gebundene Holzwolleplatten (Monoplatten der Baustoffklasse A2).pdf"}]}, "type": "source data set", "uuid": {"uuid": "027813fe-834f-45b2-8c54-86e8c8e55faf"}, "refObjectId": "027813fe-834f-45b2-8c54-86e8c8e55faf", "resourceURLs": ["https://oekobaudat.de/OEKOBAU.DAT/resource/sources/027813fe-834f-45b2-8c54-86e8c8e55faf/Fibrolith_mineralisch_gebundene_Holzwolleplatten_Monoplatten_der_Baustoffklasse_A2__17881.pdf?version=00.01.000"]}}]}}, "validation": {"review": [{"referenceToNameOfReviewerAndInstitution": [{"shortDescription": [{"value": "Institut Bauen und Umwelt e. V.", "lang": "de"}], "type": "contact data set", "refObjectId": "d111dbec-b024-4be5-86c5-752d6eb2cf95", "uri": "../contacts/d111dbec-b024-4be5-86c5-752d6eb2cf95.xml"}], "type": "Accredited third party review"}]}, "complianceDeclarations": {"compliance": [{"referenceToComplianceSystem": {"shortDescription": [{"value": "DIN EN 15804+A2", "lang": "de"}], "type": "source data set", "refObjectId": "c0016b33-8cf7-415c-ac6e-deba0d21440d", "uri": "../sources/c0016b33-8cf7-415c-ac6e-deba0d21440d.xml"}}, {"referenceToComplianceSystem": {"shortDescription": [{"value": "ISO 14025", "lang": "de"}], "type": "source data set", "refObjectId": "4f2eb655-6e44-4874-a95a-e28f5442cd4d", "uri": "../sources/4f2eb655-6e44-4874-a95a-e28f5442cd4d.xml"}}]}}, "administrativeInformation": {"commissionerAndGoal": {"referenceToCommissioner": [{"shortDescription": [{"value": "Fibrolith Dämmstoffe GmbH", "lang": "de"}], "type": "contact data set", "refObjectId": "509d3926-eea6-493f-89ff-9e22ca9eb5c7", "uri": "../contacts/509d3926-eea6-493f-89ff-9e22ca9eb5c7.xml"}]}, "dataGenerator": {"referenceToPersonOrEntityGeneratingTheDataSet": [{"shortDescription": [{"value": "Dr. Frank Werner - Umwelt & Entwicklung", "lang": "de"}], "type": "contact data set", "refObjectId": "62792478-795c-4ae2-ac9a-1012d9515424", "uri": "../contacts/62792478-795c-4ae2-ac9a-1012d9515424.xml"}]}, "dataEntryBy": {"timeStamp": 1707955200000, "referenceToDataSetFormat": [{"shortDescription": [{"value": "ILCD Format", "lang": "de"}], "type": "source data set", "refObjectId": "a97a0155-0234-4b87-b4ce-a45da52f2a40", "uri": "../sources/a97a0155-0234-4b87-b4ce-a45da52f2a40.xml"}, {"shortDescription": [{"value": "EPD-Datenformaterweiterungen v1.2", "lang": "de"}, {"value": "EPD Data Format Extensions v1.2", "lang": "en"}], "type": "source data set", "refObjectId": "a29449fd-aa2f-4de8-b5d7-4b06b43c6fde", "uri": "../sources/a29449fd-aa2f-4de8-b5d7-4b06b43c6fde.xml"}]}, "publicationAndOwnership": {"dataSetVersion": "00.01.000", "referenceToRegistrationAuthority": {"shortDescription": [{"value": "Institut Bauen und Umwelt e. V.", "lang": "de"}], "type": "contact data set", "refObjectId": "d111dbec-b024-4be5-86c5-752d6eb2cf95", "uri": "../contacts/d111dbec-b024-4be5-86c5-752d6eb2cf95.xml"}, "registrationNumber": "EPD-FIB-20230464-IBC1-DE", "referenceToOwnershipOfDataSet": {"shortDescription": [{"value": "Fibrolith Dämmstoffe GmbH", "lang": "de"}], "type": "contact data set", "refObjectId": "509d3926-eea6-493f-89ff-9e22ca9eb5c7", "uri": "../contacts/509d3926-eea6-493f-89ff-9e22ca9eb5c7.xml"}, "copyright": true, "licenseType": "Free of charge for all users and uses", "accessRestrictions": [{"value": "None", "lang": "en"}], "other": {"anies": [{"name": "referenceToPublisher", "value": {"shortDescription": [{"value": "Institut Bauen und Umwelt e. V.", "lang": "de"}], "type": "contact data set", "refObjectId": "d111dbec-b024-4be5-86c5-752d6eb2cf95", "uri": "../contacts/d111dbec-b024-4be5-86c5-752d6eb2cf95.xml"}}]}}}, "exchanges": {"exchange": [{"dataSetInternalID": 0, "referenceToFlowDataSet": {"shortDescription": [{"value": "fibrolith® zementgebundene Holzwolleplatten (Monoplatten der Baustoffklasse A2) ()", "lang": "de"}], "type": "flow data set", "refObjectId": "04fd4e92-720c-ff49-0221-4ac58b8d484c", "uri": "../flows/04fd4e92-720c-ff49-0221-4ac58b8d484c.xml"}, "meanAmount": 1.0, "referencesToDataSource": {}, "referenceFlow": true, "resolvedFlowVersion": "00.01.000", "resultingflowAmount": 1000.0, "flowProperties": [{"name": [{"lang": "en", "value": "Mass"}, {"lang": "de", "value": "Masse"}], "uuid": "93a60a56-a3c8-11da-a746-0800200b9a66", "referenceFlowProperty": true, "meanValue": 1000.0, "referenceUnit": "kg", "unitGroupUUID": "ad38d542-3fe9-439d-9b95-2f5f7752acaf"}], "materialProperties": [{"name": "gross density", "value": "494.4", "unit": "kg/m^3", "unitDescription": "kilograms per cubic metre"}], "typeOfFlow": "Product flow", "classification": {"classHierarchy": "Dämmstoffe / Holzwolleplatten / Holzwolleleichtbauplatten", "name": "OEKOBAU.DAT"}}, {"dataSetInternalID": 1, "referenceToFlowDataSet": {"shortDescription": [{"value": "Erneuerbare Primärenergie als Energieträger (PERE)", "lang": "de"}, {"value": "Renewable primary energy as energy carrier (PERE)", "lang": "en"}], "type": "flow data set", "refObjectId": "20f32be5-0398-4288-9b6d-accddd195317", "uri": "../flows/20f32be5-0398-4288-9b6d-accddd195317.xml"}, "exchange direction": "INPUT", "other": {"anies": [{"name": "referenceToUnitGroupDataSet", "value": {"shortDescription": [{"value": "MJ", "lang": "de"}], "type": "unit group data set", "refObjectId": "93a60a57-a3c8-11da-a746-0800200c9a66", "uri": "../unitgroups/93a60a57-a3c8-11da-a746-0800200c9a66.xml"}}, {"value": "1751.30542946779", "module": "A1-A3"}, {"value": "201.717968326395", "module": "A5"}, {"module": "B1"}, {"value": "0", "module": "C1"}, {"value": "2.02908155146321", "module": "C2"}, {"value": "7678.0893800175", "module": "C3"}, {"value": "0", "module": "C4"}, {"value": "-458.50263652527", "module": "D"}]}, "resolvedFlowVersion": "38.00.000", "flowProperties": [], "typeOfFlow": "Other flow", "classification": {"classHierarchy": "Quantities", "name": "GaBiCategories"}}, {"dataSetInternalID": 2, "referenceToFlowDataSet": {"shortDescription": [{"value": "Erneuerbare Primärenergie zur stofflichen Nutzung (PERM)", "lang": "de"}, {"value": "Renewable primary energy resources as material utilization (PERM)", "lang": "en"}], "type": "flow data set", "refObjectId": "fb3ec0de-548d-4508-aea5-00b73bf6f702", "uri": "../flows/fb3ec0de-548d-4508-aea5-00b73bf6f702.xml"}, "exchange direction": "INPUT", "other": {"anies": [{"name": "referenceToUnitGroupDataSet", "value": {"shortDescription": [{"value": "MJ", "lang": "de"}], "type": "unit group data set", "refObjectId": "93a60a57-a3c8-11da-a746-0800200c9a66", "uri": "../unitgroups/93a60a57-a3c8-11da-a746-0800200c9a66.xml"}}, {"value": "7873.71241747573", "module": "A1-A3"}, {"value": "-201.644417475728", "module": "A5"}, {"module": "B1"}, {"value": "0", "module": "C1"}, {"value": "0", "module": "C2"}, {"value": "-7672.068", "module": "C3"}, {"value": "0", "module": "C4"}, {"value": "0", "module": "D"}]}, "resolvedFlowVersion": "38.00.000", "flowProperties": [], "typeOfFlow": "Other flow", "classification": {"classHierarchy": "Quantities", "name": "GaBiCategories"}}, {"dataSetInternalID": 3, "referenceToFlowDataSet": {"shortDescription": [{"value": "Total erneuerbare Primärenergie (PERT)", "lang": "de"}, {"value": "Total use of renewable primary energy resources (PERT)", "lang": "en"}], "type": "flow data set", "refObjectId": "53f97275-fa8a-4cdd-9024-65936002acd0", "uri": "../flows/53f97275-fa8a-4cdd-9024-65936002acd0.xml"}, "exchange direction": "INPUT", "other": {"anies": [{"name": "referenceToUnitGroupDataSet", "value": {"shortDescription": [{"value": "MJ", "lang": "de"}], "type": "unit group data set", "refObjectId": "93a60a57-a3c8-11da-a746-0800200c9a66", "uri": "../unitgroups/93a60a57-a3c8-11da-a746-0800200c9a66.xml"}}, {"value": "9625.01784694352", "module": "A1-A3"}, {"value": "0.0735508506667721", "module": "A5"}, {"module": "B1"}, {"value": "0", "module": "C1"}, {"value": "2.02908155146321", "module": "C2"}, {"value": "6.02138001749598", "module": "C3"}, {"value": "0", "module": "C4"}, {"value": "-458.50263652527", "module": "D"}]}, "resolvedFlowVersion": "38.00.000", "flowProperties": [], "typeOfFlow": "Other flow", "classification": {"classHierarchy": "Quantities / Environmental quantities / EPD EN 15804 / LCI indicators", "name": "GaBiCategories"}}, {"dataSetInternalID": 4, "referenceToFlowDataSet": {"shortDescription": [{"value": "Nicht-erneuerbare Primärenergie als Energieträger (PENRE)", "lang": "de"}, {"value": "Non renewable primary energy as energy carrier (PENRE)", "lang": "en"}], "type": "flow data set", "refObjectId": "ac857178-2b45-46ec-892a-a9a4332f0372", "uri": "../flows/ac857178-2b45-46ec-892a-a9a4332f0372.xml"}, "exchange direction": "INPUT", "other": {"anies": [{"name": "referenceToUnitGroupDataSet", "value": {"shortDescription": [{"value": "MJ", "lang": "de"}], "type": "unit group data set", "refObjectId": "93a60a57-a3c8-11da-a746-0800200c9a66", "uri": "../unitgroups/93a60a57-a3c8-11da-a746-0800200c9a66.xml"}}, {"value": "6309.95157461827", "module": "A1-A3"}, {"value": "12.6490109659091", "module": "A5"}, {"module": "B1"}, {"value": "0", "module": "C1"}, {"value": "131.244679417595", "module": "C2"}, {"value": "228.255986409239", "module": "C3"}, {"value": "0", "module": "C4"}, {"value": "-4532.06953211785", "module": "D"}]}, "resolvedFlowVersion": "38.00.000", "flowProperties": [], "typeOfFlow": "Other flow", "classification": {"classHierarchy": "Quantities", "name": "GaBiCategories"}}, {"dataSetInternalID": 5, "referenceToFlowDataSet": {"shortDescription": [{"value": "Nicht-erneuerbare Primärenergie zur stofflichen Nutzung (PENRM)", "lang": "de"}, {"value": "Non renewable primary energy as material utilization (PENRM)", "lang": "en"}], "type": "flow data set", "refObjectId": "1421caa0-679d-4bf4-b282-0eb850ccae27", "uri": "../flows/1421caa0-679d-4bf4-b282-0eb850ccae27.xml"}, "exchange direction": "INPUT", "other": {"anies": [{"name": "referenceToUnitGroupDataSet", "value": {"shortDescription": [{"value": "MJ", "lang": "de"}], "type": "unit group data set", "refObjectId": "93a60a57-a3c8-11da-a746-0800200c9a66", "uri": "../unitgroups/93a60a57-a3c8-11da-a746-0800200c9a66.xml"}}, {"value": "9.59417475728156", "module": "A1-A3"}, {"value": "-9.59417475728156", "module": "A5"}, {"module": "B1"}, {"value": "0", "module": "C1"}, {"value": "0", "module": "C2"}, {"value": "0", "module": "C3"}, {"value": "0", "module": "C4"}, {"value": "0", "module": "D"}]}, "resolvedFlowVersion": "38.00.000", "flowProperties": [], "typeOfFlow": "Other flow", "classification": {"classHierarchy": "Quantities", "name": "GaBiCategories"}}, {"dataSetInternalID": 6, "referenceToFlowDataSet": {"shortDescription": [{"value": "Total nicht erneuerbare Primärenergie (PENRT)", "lang": "de"}, {"value": "Total use of non renewable primary energy resources (PENRT)", "lang": "en"}], "type": "flow data set", "refObjectId": "06159210-646b-4c8d-8583-da9b3b95a6c1", "uri": "../flows/06159210-646b-4c8d-8583-da9b3b95a6c1.xml"}, "exchange direction": "INPUT", "other": {"anies": [{"name": "referenceToUnitGroupDataSet", "value": {"shortDescription": [{"value": "MJ", "lang": "de"}], "type": "unit group data set", "refObjectId": "93a60a57-a3c8-11da-a746-0800200c9a66", "uri": "../unitgroups/93a60a57-a3c8-11da-a746-0800200c9a66.xml"}}, {"value": "6319.54574937555", "module": "A1-A3"}, {"value": "3.05483620862752", "module": "A5"}, {"module": "B1"}, {"value": "0", "module": "C1"}, {"value": "131.244679417595", "module": "C2"}, {"value": "228.255986409239", "module": "C3"}, {"value": "0", "module": "C4"}, {"value": "-4532.06953211785", "module": "D"}]}, "resolvedFlowVersion": "38.00.000", "flowProperties": [], "typeOfFlow": "Other flow", "classification": {"classHierarchy": "Quantities / Environmental quantities / EPD EN 15804 / LCI indicators", "name": "GaBiCategories"}}, {"dataSetInternalID": 7, "referenceToFlowDataSet": {"shortDescription": [{"value": "Einsatz von Sekundärstoffen (SM)", "lang": "de"}, {"value": "Use of secondary material (SM)", "lang": "en"}], "type": "flow data set", "refObjectId": "c6a1f35f-2d09-4f54-8dfb-97e502e1ce92", "uri": "../flows/c6a1f35f-2d09-4f54-8dfb-97e502e1ce92.xml"}, "exchange direction": "INPUT", "other": {"anies": [{"name": "referenceToUnitGroupDataSet", "value": {"shortDescription": [{"value": "kg", "lang": "de"}], "type": "unit group data set", "refObjectId": "ad38d542-3fe9-439d-9b95-2f5f7752acaf", "uri": "../unitgroups/ad38d542-3fe9-439d-9b95-2f5f7752acaf.xml"}}, {"value": "1.58171521035599", "module": "A1-A3"}, {"value": "0", "module": "A5"}, {"module": "B1"}, {"value": "0", "module": "C1"}, {"value": "0", "module": "C2"}, {"value": "0", "module": "C3"}, {"value": "0", "module": "C4"}, {"value": "0", "module": "D"}]}, "resolvedFlowVersion": "38.00.000", "flowProperties": [], "typeOfFlow": "Other flow", "classification": {"classHierarchy": "Quantities / Environmental quantities / EPD EN 15804 / LCI indicators", "name": "GaBiCategories"}}, {"dataSetInternalID": 8, "referenceToFlowDataSet": {"shortDescription": [{"value": "Erneuerbare Sekundärbrennstoffe (RSF)", "lang": "de"}, {"value": "Use of renewable secondary fuels (RSF)", "lang": "en"}], "type": "flow data set", "refObjectId": "64333088-a55f-4aa2-9a31-c10b07816787", "uri": "../flows/64333088-a55f-4aa2-9a31-c10b07816787.xml"}, "exchange direction": "INPUT", "other": {"anies": [{"name": "referenceToUnitGroupDataSet", "value": {"shortDescription": [{"value": "MJ", "lang": "de"}], "type": "unit group data set", "refObjectId": "93a60a57-a3c8-11da-a746-0800200c9a66", "uri": "../unitgroups/93a60a57-a3c8-11da-a746-0800200c9a66.xml"}}, {"value": "0", "module": "A1-A3"}, {"value": "0", "module": "A5"}, {"module": "B1"}, {"value": "0", "module": "C1"}, {"value": "0", "module": "C2"}, {"value": "0", "module": "C3"}, {"value": "0", "module": "C4"}, {"value": "0", "module": "D"}]}, "resolvedFlowVersion": "38.00.000", "flowProperties": [], "typeOfFlow": "Other flow", "classification": {"classHierarchy": "Quantities / Environmental quantities / EPD EN 15804 / LCI indicators", "name": "GaBiCategories"}}, {"dataSetInternalID": 9, "referenceToFlowDataSet": {"shortDescription": [{"value": "Nicht erneuerbare Sekundärbrennstoffe (NRSF)", "lang": "de"}, {"value": "Use of non renewable secondary fuels (NRSF)", "lang": "en"}], "type": "flow data set", "refObjectId": "89def144-d39a-4287-b86f-efde453ddcb2", "uri": "../flows/89def144-d39a-4287-b86f-efde453ddcb2.xml"}, "exchange direction": "INPUT", "other": {"anies": [{"name": "referenceToUnitGroupDataSet", "value": {"shortDescription": [{"value": "MJ", "lang": "de"}], "type": "unit group data set", "refObjectId": "93a60a57-a3c8-11da-a746-0800200c9a66", "uri": "../unitgroups/93a60a57-a3c8-11da-a746-0800200c9a66.xml"}}, {"value": "0", "module": "A1-A3"}, {"value": "0", "module": "A5"}, {"module": "B1"}, {"value": "0", "module": "C1"}, {"value": "0", "module": "C2"}, {"value": "0", "module": "C3"}, {"value": "0", "module": "C4"}, {"value": "0", "module": "D"}]}, "resolvedFlowVersion": "38.00.000", "flowProperties": [], "typeOfFlow": "Other flow", "classification": {"classHierarchy": "Quantities / Environmental quantities / EPD EN 15804 / LCI indicators", "name": "GaBiCategories"}}, {"dataSetInternalID": 10, "referenceToFlowDataSet": {"shortDescription": [{"value": "Einsatz von Süßwasserressourcen (FW)", "lang": "de"}, {"value": "Use of net fresh water (FW)", "lang": "en"}], "type": "flow data set", "refObjectId": "3cf952c8-f3a4-461d-8c96-96456ca62246", "uri": "../flows/3cf952c8-f3a4-461d-8c96-96456ca62246.xml"}, "exchange direction": "INPUT", "other": {"anies": [{"name": "referenceToUnitGroupDataSet", "value": {"shortDescription": [{"value": "m^3", "lang": "de"}], "type": "unit group data set", "refObjectId": "cd950537-0a98-4044-9ba7-9f9a68d0a504", "uri": "../unitgroups/cd950537-0a98-4044-9ba7-9f9a68d0a504.xml"}}, {"value": "2.03836482532931", "module": "A1-A3"}, {"value": "0.0108650955023644", "module": "A5"}, {"module": "B1"}, {"value": "0", "module": "C1"}, {"value": "0.034321450228145", "module": "C2"}, {"value": "0.444242279595565", "module": "C3"}, {"value": "0", "module": "C4"}, {"value": "-0.86383069022495", "module": "D"}]}, "resolvedFlowVersion": "38.00.000", "flowProperties": [], "typeOfFlow": "Other flow", "classification": {"classHierarchy": "Quantities / Environmental quantities / EPD EN 15804 / LCI indicators", "name": "GaBiCategories"}}, {"dataSetInternalID": 11, "referenceToFlowDataSet": {"shortDescription": [{"value": "Gefährlicher Abfall zur Deponie (HWD)", "lang": "de"}, {"value": "Hazardous waste disposed (HWD)", "lang": "en"}], "type": "flow data set", "refObjectId": "430f9e0f-59b2-46a0-8e0d-55e0e84948fc", "uri": "../flows/430f9e0f-59b2-46a0-8e0d-55e0e84948fc.xml"}, "exchange direction": "OUTPUT", "other": {"anies": [{"name": "referenceToUnitGroupDataSet", "value": {"shortDescription": [{"value": "kg", "lang": "de"}], "type": "unit group data set", "refObjectId": "ad38d542-3fe9-439d-9b95-2f5f7752acaf", "uri": "../unitgroups/ad38d542-3fe9-439d-9b95-2f5f7752acaf.xml"}}, {"value": "0.0204328035408181", "module": "A1-A3"}, {"value": "3.97089200485545E-05", "module": "A5"}, {"module": "B1"}, {"value": "0", "module": "C1"}, {"value": "0.000834676084132482", "module": "C2"}, {"value": "0.00198094991717937", "module": "C3"}, {"value": "0", "module": "C4"}, {"value": "-0.0121242388141219", "module": "D"}]}, "resolvedFlowVersion": "38.00.000", "flowProperties": [], "typeOfFlow": "Other flow", "classification": {"classHierarchy": "Quantities / Environmental quantities / EPD EN 15804 / LCI indicators", "name": "GaBiCategories"}}, {"dataSetInternalID": 12, "referenceToFlowDataSet": {"shortDescription": [{"value": "Entsorgter nicht gefährlicher Abfall (NHWD)", "lang": "de"}, {"value": "Non hazardous waste disposed (NHWD)", "lang": "en"}], "type": "flow data set", "refObjectId": "b29ef66b-e286-4afa-949f-62f1a7b4d7fa", "uri": "../flows/b29ef66b-e286-4afa-949f-62f1a7b4d7fa.xml"}, "exchange direction": "OUTPUT", "other": {"anies": [{"name": "referenceToUnitGroupDataSet", "value": {"shortDescription": [{"value": "kg", "lang": "de"}], "type": "unit group data set", "refObjectId": "ad38d542-3fe9-439d-9b95-2f5f7752acaf", "uri": "../unitgroups/ad38d542-3fe9-439d-9b95-2f5f7752acaf.xml"}}, {"value": "87.2929924242124", "module": "A1-A3"}, {"value": "0.29348836042988", "module": "A5"}, {"module": "B1"}, {"value": "0", "module": "C1"}, {"value": "6.57004624236663", "module": "C2"}, {"value": "438.009414348323", "module": "C3"}, {"value": "0", "module": "C4"}, {"value": "-12.6734748595893", "module": "D"}]}, "resolvedFlowVersion": "38.00.000", "flowProperties": [], "typeOfFlow": "Other flow", "classification": {"classHierarchy": "Quantities / Environmental quantities / EPD EN 15804 / LCI indicators", "name": "GaBiCategories"}}, {"dataSetInternalID": 13, "referenceToFlowDataSet": {"shortDescription": [{"value": "Entsorgter radioaktiver Abfall (RWD)", "lang": "de"}, {"value": "Radioactive waste disposed (RWD)", "lang": "en"}], "type": "flow data set", "refObjectId": "3449546e-52ad-4b39-b809-9fb77cea8ff6", "uri": "../flows/3449546e-52ad-4b39-b809-9fb77cea8ff6.xml"}, "exchange direction": "OUTPUT", "other": {"anies": [{"name": "referenceToUnitGroupDataSet", "value": {"shortDescription": [{"value": "kg", "lang": "de"}], "type": "unit group data set", "refObjectId": "ad38d542-3fe9-439d-9b95-2f5f7752acaf", "uri": "../unitgroups/ad38d542-3fe9-439d-9b95-2f5f7752acaf.xml"}}, {"value": "0.0247772049956812", "module": "A1-A3"}, {"value": "2.21455398539634E-06", "module": "A5"}, {"module": "B1"}, {"value": "0", "module": "C1"}, {"value": "7.52926624499602E-05", "module": "C2"}, {"value": "0.000156817880973447", "module": "C3"}, {"value": "0", "module": "C4"}, {"value": "-0.0196445460902193", "module": "D"}]}, "resolvedFlowVersion": "38.00.000", "flowProperties": [], "typeOfFlow": "Other flow", "classification": {"classHierarchy": "Quantities / Environmental quantities / EPD EN 15804 / LCI indicators", "name": "GaBiCategories"}}, {"dataSetInternalID": 14, "referenceToFlowDataSet": {"shortDescription": [{"value": "Komponenten für die Wiederverwendung (CRU)", "lang": "de"}, {"value": "Components for re-use (CRU)", "lang": "en"}], "type": "flow data set", "refObjectId": "a2b32f97-3fc7-4af2-b209-525bc6426f33", "uri": "../flows/a2b32f97-3fc7-4af2-b209-525bc6426f33.xml"}, "exchange direction": "OUTPUT", "other": {"anies": [{"name": "referenceToUnitGroupDataSet", "value": {"shortDescription": [{"value": "kg", "lang": "de"}], "type": "unit group data set", "refObjectId": "ad38d542-3fe9-439d-9b95-2f5f7752acaf", "uri": "../unitgroups/ad38d542-3fe9-439d-9b95-2f5f7752acaf.xml"}}, {"value": "0", "module": "A1-A3"}, {"value": "0", "module": "A5"}, {"module": "B1"}, {"value": "0", "module": "C1"}, {"value": "0", "module": "C2"}, {"value": "0", "module": "C3"}, {"value": "0", "module": "C4"}, {"value": "0", "module": "D"}]}, "resolvedFlowVersion": "38.00.000", "flowProperties": [], "typeOfFlow": "Other flow", "classification": {"classHierarchy": "Quantities / Environmental quantities / EPD EN 15804 / LCI indicators", "name": "GaBiCategories"}}, {"dataSetInternalID": 15, "referenceToFlowDataSet": {"shortDescription": [{"value": "Stoffe zum Recycling (MFR)", "lang": "de"}, {"value": "Materials for recycling (MFR)", "lang": "en"}], "type": "flow data set", "refObjectId": "d7fe48a5-4103-49c8-9aae-b0b5dfdbd6ae", "uri": "../flows/d7fe48a5-4103-49c8-9aae-b0b5dfdbd6ae.xml"}, "exchange direction": "OUTPUT", "other": {"anies": [{"name": "referenceToUnitGroupDataSet", "value": {"shortDescription": [{"value": "kg", "lang": "de"}], "type": "unit group data set", "refObjectId": "ad38d542-3fe9-439d-9b95-2f5f7752acaf", "uri": "../unitgroups/ad38d542-3fe9-439d-9b95-2f5f7752acaf.xml"}}, {"value": "0", "module": "A1-A3"}, {"value": "0", "module": "A5"}, {"module": "B1"}, {"value": "0", "module": "C1"}, {"value": "0", "module": "C2"}, {"value": "0", "module": "C3"}, {"value": "0", "module": "C4"}, {"value": "0", "module": "D"}]}, "resolvedFlowVersion": "38.00.000", "flowProperties": [], "typeOfFlow": "Other flow", "classification": {"classHierarchy": "Quantities / Environmental quantities / EPD EN 15804 / LCI indicators", "name": "GaBiCategories"}}, {"dataSetInternalID": 16, "referenceToFlowDataSet": {"shortDescription": [{"value": "Stoffe für die Energierückgewinnung (MER)", "lang": "de"}, {"value": "Materials for energy recovery (MER)", "lang": "en"}], "type": "flow data set", "refObjectId": "59a9181c-3aaf-46ee-8b13-2b3723b6e447", "uri": "../flows/59a9181c-3aaf-46ee-8b13-2b3723b6e447.xml"}, "exchange direction": "OUTPUT", "other": {"anies": [{"name": "referenceToUnitGroupDataSet", "value": {"shortDescription": [{"value": "kg", "lang": "de"}], "type": "unit group data set", "refObjectId": "ad38d542-3fe9-439d-9b95-2f5f7752acaf", "uri": "../unitgroups/ad38d542-3fe9-439d-9b95-2f5f7752acaf.xml"}}, {"value": "0", "module": "A1-A3"}, {"value": "0", "module": "A5"}, {"module": "B1"}, {"value": "0", "module": "C1"}, {"value": "0", "module": "C2"}, {"value": "0", "module": "C3"}, {"value": "0", "module": "C4"}, {"value": "0", "module": "D"}]}, "resolvedFlowVersion": "38.00.000", "flowProperties": [], "typeOfFlow": "Other flow", "classification": {"classHierarchy": "Quantities / Environmental quantities / EPD EN 15804 / LCI indicators", "name": "GaBiCategories"}}, {"dataSetInternalID": 17, "referenceToFlowDataSet": {"shortDescription": [{"value": "Exportierte elektrische Energie (EEE)", "lang": "de"}, {"value": "Exported electrical energy (EEE)", "lang": "en"}], "type": "flow data set", "refObjectId": "4da0c987-2b76-40d6-9e9e-82a017aaaf29", "uri": "../flows/4da0c987-2b76-40d6-9e9e-82a017aaaf29.xml"}, "exchange direction": "OUTPUT", "other": {"anies": [{"name": "referenceToUnitGroupDataSet", "value": {"shortDescription": [{"value": "MJ", "lang": "de"}], "type": "unit group data set", "refObjectId": "93a60a57-a3c8-11da-a746-0800200c9a66", "uri": "../unitgroups/93a60a57-a3c8-11da-a746-0800200c9a66.xml"}}, {"value": "0", "module": "A1-A3"}, {"value": "30.8879233009708", "module": "A5"}, {"module": "B1"}, {"value": "0", "module": "C1"}, {"value": "0", "module": "C2"}, {"value": "1120.20756", "module": "C3"}, {"value": "0", "module": "C4"}, {"value": "0", "module": "D"}]}, "resolvedFlowVersion": "38.00.000", "flowProperties": [], "typeOfFlow": "Other flow", "classification": {"classHierarchy": "Quantities / Environmental quantities / EPD EN 15804 / LCI indicators", "name": "GaBiCategories"}}, {"dataSetInternalID": 18, "referenceToFlowDataSet": {"shortDescription": [{"value": "Exportierte thermische Energie (EET)", "lang": "de"}, {"value": "Exported thermal energy (EET)", "lang": "en"}], "type": "flow data set", "refObjectId": "98daf38a-7a79-46d3-9a37-2b7bd0955810", "uri": "../flows/98daf38a-7a79-46d3-9a37-2b7bd0955810.xml"}, "exchange direction": "OUTPUT", "other": {"anies": [{"name": "referenceToUnitGroupDataSet", "value": {"shortDescription": [{"value": "MJ", "lang": "de"}], "type": "unit group data set", "refObjectId": "93a60a57-a3c8-11da-a746-0800200c9a66", "uri": "../unitgroups/93a60a57-a3c8-11da-a746-0800200c9a66.xml"}}, {"value": "0", "module": "A1-A3"}, {"value": "59.0627182038834", "module": "A5"}, {"module": "B1"}, {"value": "0", "module": "C1"}, {"value": "0", "module": "C2"}, {"value": "2142.01851", "module": "C3"}, {"value": "0", "module": "C4"}, {"value": "0", "module": "D"}]}, "resolvedFlowVersion": "38.00.000", "flowProperties": [], "typeOfFlow": "Other flow", "classification": {"classHierarchy": "Quantities / Environmental quantities / EPD EN 15804 / LCI indicators", "name": "GaBiCategories"}}]}, "LCIAResults": {"LCIAResult": [{"referenceToLCIAMethodDataSet": {"shortDescription": [{"value": "Globales Erwärmungspotenzial total (GWP-total)", "lang": "de"}, {"value": "Global Warming Potential total (GWP-total)", "lang": "en"}], "type": "LCIA method data set", "refObjectId": "6a37f984-a4b3-458a-a20a-64418c145fa2", "uri": "../lciamethods/6a37f984-a4b3-458a-a20a-64418c145fa2.xml"}, "other": {"anies": [{"name": "referenceToUnitGroupDataSet", "value": {"shortDescription": [{"value": "kg CO_(2)-Äq.", "lang": "de"}], "type": "unit group data set", "refObjectId": "1ebf3012-d0db-4de2-aefd-ef30cedb0be1", "uri": "../unitgroups/1ebf3012-d0db-4de2-aefd-ef30cedb0be1.xml"}}, {"value": "146.979486415176", "module": "A1-A3"}, {"value": "20.3294895108396", "module": "A5"}, {"value": "-254.8", "module": "B1"}, {"value": "0", "module": "C1"}, {"value": "9.48149842702543", "module": "C2"}, {"value": "753.86800227932", "module": "C3"}, {"value": "0", "module": "C4"}, {"value": "-309.604898087939", "module": "D"}]}}, {"referenceToLCIAMethodDataSet": {"shortDescription": [{"value": "Globales Erwärmungspotenzial fossil (GWP-fossil)", "lang": "de"}, {"value": "Global Warming Potential fossil fuels (GWP-fossil)", "lang": "en"}], "type": "LCIA method data set", "refObjectId": "5f635281-343e-44fb-83df-1971b155e6b6", "uri": "../lciamethods/5f635281-343e-44fb-83df-1971b155e6b6.xml"}, "other": {"anies": [{"name": "referenceToUnitGroupDataSet", "value": {"shortDescription": [{"value": "kg CO_(2)-Äq.", "lang": "de"}], "type": "unit group data set", "refObjectId": "1ebf3012-d0db-4de2-aefd-ef30cedb0be1", "uri": "../unitgroups/1ebf3012-d0db-4de2-aefd-ef30cedb0be1.xml"}}, {"value": "902.367337110472", "module": "A1-A3"}, {"value": "0.954058002700918", "module": "A5"}, {"value": "-254.8", "module": "B1"}, {"value": "0", "module": "C1"}, {"value": "9.4769010164487", "module": "C2"}, {"value": "16.6796285906613", "module": "C3"}, {"value": "0", "module": "C4"}, {"value": "-309.34479214456", "module": "D"}]}}, {"referenceToLCIAMethodDataSet": {"shortDescription": [{"value": "Globales Erwärmungspotenzial biogen (GWP-biogenic)", "lang": "de"}, {"value": "Global Warming Potential biogenic (GWP-biogenic)", "lang": "en"}], "type": "LCIA method data set", "refObjectId": "2356e1ab-0185-4db5-86e5-16de51c7485c", "uri": "../lciamethods/2356e1ab-0185-4db5-86e5-16de51c7485c.xml"}, "other": {"anies": [{"name": "referenceToUnitGroupDataSet", "value": {"shortDescription": [{"value": "kg CO_(2)-Äq.", "lang": "de"}], "type": "unit group data set", "refObjectId": "1ebf3012-d0db-4de2-aefd-ef30cedb0be1", "uri": "../unitgroups/1ebf3012-d0db-4de2-aefd-ef30cedb0be1.xml"}}, {"value": "-756.558670442287", "module": "A1-A3"}, {"value": "19.3753371089536", "module": "A5"}, {"module": "B1"}, {"value": "0", "module": "C1"}, {"value": "0", "module": "C2"}, {"value": "737.183333333333", "module": "C3"}, {"value": "0", "module": "C4"}, {"value": "0", "module": "D"}]}}, {"referenceToLCIAMethodDataSet": {"shortDescription": [{"value": "Globales Erwärmungspotenzial luluc (GWP-luluc)", "lang": "de"}, {"value": "Global Warming Potential luluc (GWP-luluc)", "lang": "en"}], "type": "LCIA method data set", "refObjectId": "4331bbdb-978a-490d-8707-eeb047f01a55", "uri": "../lciamethods/4331bbdb-978a-490d-8707-eeb047f01a55.xml"}, "other": {"anies": [{"name": "referenceToUnitGroupDataSet", "value": {"shortDescription": [{"value": "kg CO_(2)-Äq.", "lang": "de"}], "type": "unit group data set", "refObjectId": "1ebf3012-d0db-4de2-aefd-ef30cedb0be1", "uri": "../unitgroups/1ebf3012-d0db-4de2-aefd-ef30cedb0be1.xml"}}, {"value": "1.17081974699112", "module": "A1-A3"}, {"value": "9.43991851178439E-05", "module": "A5"}, {"module": "B1"}, {"value": "0", "module": "C1"}, {"value": "0.00459741057673308", "module": "C2"}, {"value": "0.00504035532568158", "module": "C3"}, {"value": "0", "module": "C4"}, {"value": "-0.260105943379047", "module": "D"}]}}, {"referenceToLCIAMethodDataSet": {"shortDescription": [{"value": "Abbau Potential der stratosphärischen Ozonschicht (ODP)", "lang": "de"}, {"value": "Depletion potential of the stratospheric ozone layer (ODP)", "lang": "en"}], "type": "LCIA method data set", "refObjectId": "b5c629d6-def3-11e6-bf01-fe55135034f3", "uri": "../lciamethods/b5c629d6-def3-11e6-bf01-fe55135034f3.xml"}, "other": {"anies": [{"name": "referenceToUnitGroupDataSet", "value": {"shortDescription": [{"value": "kg CFC11-Äq.", "lang": "de"}], "type": "unit group data set", "refObjectId": "d9e957c9-7309-4474-bf3a-7777df6c4e5b", "uri": "../unitgroups/d9e957c9-7309-4474-bf3a-7777df6c4e5b.xml"}}, {"value": "8.79158498164281E-06", "module": "A1-A3"}, {"value": "6.65768167167094E-09", "module": "A5"}, {"module": "B1"}, {"value": "0", "module": "C1"}, {"value": "2.01083868735671E-07", "module": "C2"}, {"value": "3.8633623480472E-07", "module": "C3"}, {"value": "0", "module": "C4"}, {"value": "-8.41001670101561E-06", "module": "D"}]}}, {"referenceToLCIAMethodDataSet": {"shortDescription": [{"value": "Versauerungspotenzial von Boden und Wasser (AP)", "lang": "de"}, {"value": "Acidification potential of land and water (AP)", "lang": "en"}], "type": "LCIA method data set", "refObjectId": "b5c611c6-def3-11e6-bf01-fe55135034f3", "uri": "../lciamethods/b5c611c6-def3-11e6-bf01-fe55135034f3.xml"}, "other": {"anies": [{"name": "referenceToUnitGroupDataSet", "value": {"shortDescription": [{"value": "mol H^(+)-Äq.", "lang": "de"}], "type": "unit group data set", "refObjectId": "42e089ac-92bf-4bf2-8ca1-5fc40d18f2ed", "uri": "../unitgroups/42e089ac-92bf-4bf2-8ca1-5fc40d18f2ed.xml"}}, {"value": "2.12102157519331", "module": "A1-A3"}, {"value": "0.00230232897311429", "module": "A5"}, {"module": "B1"}, {"value": "0", "module": "C1"}, {"value": "0.0201934195573864", "module": "C2"}, {"value": "0.123298405607237", "module": "C3"}, {"value": "0", "module": "C4"}, {"value": "-0.427409422464771", "module": "D"}]}}, {"referenceToLCIAMethodDataSet": {"shortDescription": [{"value": "Eutrophierungspotenzial Süßwasser (EP-freshwater)", "lang": "de"}, {"value": "Eutrophication potential aquatic freshwater (EP-freshwater)", "lang": "en"}], "type": "LCIA method data set", "refObjectId": "b53ec18f-7377-4ad3-86eb-cc3f4f276b2b", "uri": "../lciamethods/b53ec18f-7377-4ad3-86eb-cc3f4f276b2b.xml"}, "other": {"anies": [{"name": "referenceToUnitGroupDataSet", "value": {"shortDescription": [{"value": "kg P-Äq.", "lang": "de"}], "type": "unit group data set", "refObjectId": "0429039d-a61d-4590-ba67-aa4a20a810a1", "uri": "../unitgroups/0429039d-a61d-4590-ba67-aa4a20a810a1.xml"}}, {"value": "0.0265538300896384", "module": "A1-A3"}, {"value": "3.74458842010805E-06", "module": "A5"}, {"module": "B1"}, {"value": "0", "module": "C1"}, {"value": "7.50419957263778E-05", "module": "C2"}, {"value": "0.000232665726996408", "module": "C3"}, {"value": "0", "module": "C4"}, {"value": "-0.0231793917817548", "module": "D"}]}}, {"referenceToLCIAMethodDataSet": {"shortDescription": [{"value": "Eutrophierungspotenzial Salzwasser (EP-marine)", "lang": "de"}, {"value": "Eutrophication potential aquatic marine (EP-marine)", "lang": "en"}], "type": "LCIA method data set", "refObjectId": "b5c619fa-def3-11e6-bf01-fe55135034f3", "uri": "../lciamethods/b5c619fa-def3-11e6-bf01-fe55135034f3.xml"}, "other": {"anies": [{"name": "referenceToUnitGroupDataSet", "value": {"shortDescription": [{"value": "kg N-Äq.", "lang": "de"}], "type": "unit group data set", "refObjectId": "d05bb823-ecdf-4686-8c40-bf1d9257859f", "uri": "../unitgroups/d05bb823-ecdf-4686-8c40-bf1d9257859f.xml"}}, {"value": "0.68721427679249", "module": "A1-A3"}, {"value": "0.00106266291172288", "module": "A5"}, {"module": "B1"}, {"value": "0", "module": "C1"}, {"value": "0.00497141709571208", "module": "C2"}, {"value": "0.0551559524446517", "module": "C3"}, {"value": "0", "module": "C4"}, {"value": "-0.0949623028166609", "module": "D"}]}}, {"referenceToLCIAMethodDataSet": {"shortDescription": [{"value": "Eutrophierungspotenzial Land (EP-terrestrial)", "lang": "de"}, {"value": "Eutrophication potential terrestrial (EP-terrestrial)", "lang": "en"}], "type": "LCIA method data set", "refObjectId": "b5c614d2-def3-11e6-bf01-fe55135034f3", "uri": "../lciamethods/b5c614d2-def3-11e6-bf01-fe55135034f3.xml"}, "other": {"anies": [{"name": "referenceToUnitGroupDataSet", "value": {"shortDescription": [{"value": "mol N-Äq.", "lang": "de"}], "type": "unit group data set", "refObjectId": "71b4d617-0ec9-4d3f-b65e-e438940c2401", "uri": "../unitgroups/71b4d617-0ec9-4d3f-b65e-e438940c2401.xml"}}, {"value": "7.70313740962775", "module": "A1-A3"}, {"value": "0.0112886433154428", "module": "A5"}, {"module": "B1"}, {"value": "0", "module": "C1"}, {"value": "0.0517637490534982", "module": "C2"}, {"value": "0.589622015751285", "module": "C3"}, {"value": "0", "module": "C4"}, {"value": "-1.14313998529078", "module": "D"}]}}, {"referenceToLCIAMethodDataSet": {"shortDescription": [{"value": "Bildungspotential für troposphärisches Ozon (POCP)", "lang": "de"}, {"value": "Formation potential of tropospheric ozone photochemical oxidants (POCP)", "lang": "en"}], "type": "LCIA method data set", "refObjectId": "b5c610fe-def3-11e6-bf01-fe55135034f3", "uri": "../lciamethods/b5c610fe-def3-11e6-bf01-fe55135034f3.xml"}, "other": {"anies": [{"name": "referenceToUnitGroupDataSet", "value": {"shortDescription": [{"value": "kg NMVOC-Äq.", "lang": "de"}], "type": "unit group data set", "refObjectId": "d27c25f8-fbc1-44c6-b47b-4adbae4199c6", "uri": "../unitgroups/d27c25f8-fbc1-44c6-b47b-4adbae4199c6.xml"}}, {"value": "2.50132459907878", "module": "A1-A3"}, {"value": "0.00308855172723043", "module": "A5"}, {"module": "B1"}, {"value": "0", "module": "C1"}, {"value": "0.0313478739374337", "module": "C2"}, {"value": "0.178079571729511", "module": "C3"}, {"value": "0", "module": "C4"}, {"value": "-0.47125761227793", "module": "D"}]}}, {"referenceToLCIAMethodDataSet": {"shortDescription": [{"value": "Potenzial für den abiotischen Abbau nicht fossiler Ressourcen (ADPE)", "lang": "de"}, {"value": "Abiotic depletion potential for non fossil resources (ADPE)", "lang": "en"}], "type": "LCIA method data set", "refObjectId": "b2ad6494-c78d-11e6-9d9d-cec0c932ce01", "uri": "../lciamethods/b2ad6494-c78d-11e6-9d9d-cec0c932ce01.xml"}, "other": {"anies": [{"name": "referenceToUnitGroupDataSet", "value": {"shortDescription": [{"value": "kg Sb-Äq.", "lang": "de"}], "type": "unit group data set", "refObjectId": "54ccd2d9-a32a-4fc2-923d-f2c8c93e89d4", "uri": "../unitgroups/54ccd2d9-a32a-4fc2-923d-f2c8c93e89d4.xml"}}, {"value": "0.000750732169282553", "module": "A1-A3"}, {"value": "6.59105909843947E-07", "module": "A5"}, {"module": "B1"}, {"value": "0", "module": "C1"}, {"value": "3.01984515407382E-05", "module": "C2"}, {"value": "3.26768898480054E-05", "module": "C3"}, {"value": "0", "module": "C4"}, {"value": "-0.000290738143939499", "module": "D"}]}}, {"referenceToLCIAMethodDataSet": {"shortDescription": [{"value": "Potenzial für den abiotischen Abbau fossiler Brennstoffe (ADPF)", "lang": "de"}, {"value": "Abiotic depletion potential for fossil resources (ADPF)", "lang": "en"}], "type": "LCIA method data set", "refObjectId": "b2ad6110-c78d-11e6-9d9d-cec0c932ce01", "uri": "../lciamethods/b2ad6110-c78d-11e6-9d9d-cec0c932ce01.xml"}, "other": {"anies": [{"name": "referenceToUnitGroupDataSet", "value": {"shortDescription": [{"value": "MJ", "lang": "de"}], "type": "unit group data set", "refObjectId": "93a60a57-a3c8-11da-a746-0800200c9a66", "uri": "../unitgroups/93a60a57-a3c8-11da-a746-0800200c9a66.xml"}}, {"value": "6315.46349329855", "module": "A1-A3"}, {"value": "3.05390102367801", "module": "A5"}, {"module": "B1"}, {"value": "0", "module": "C1"}, {"value": "131.203405388521", "module": "C2"}, {"value": "228.202712778078", "module": "C3"}, {"value": "0", "module": "C4"}, {"value": "-4483.24320233344", "module": "D"}]}}, {"referenceToLCIAMethodDataSet": {"shortDescription": [{"value": "Wassernutzung (WDP)", "lang": "de"}, {"value": "Water use (WDP)", "lang": "en"}], "type": "LCIA method data set", "refObjectId": "b2ad66ce-c78d-11e6-9d9d-cec0c932ce01", "uri": "../lciamethods/b2ad66ce-c78d-11e6-9d9d-cec0c932ce01.xml"}, "other": {"anies": [{"name": "referenceToUnitGroupDataSet", "value": {"shortDescription": [{"value": "m^(3) Welt-Äq. entzogen", "lang": "de"}], "type": "unit group data set", "refObjectId": "6ae2df01-888e-46c8-b17d-49fa3869b476", "uri": "../unitgroups/6ae2df01-888e-46c8-b17d-49fa3869b476.xml"}}, {"value": "109.097422720133", "module": "A1-A3"}, {"value": "0.0348231284845055", "module": "A5"}, {"module": "B1"}, {"value": "0", "module": "C1"}, {"value": "0.548450765222039", "module": "C2"}, {"value": "2.11256814222834", "module": "C3"}, {"value": "0", "module": "C4"}, {"value": "-8.20047228436137", "module": "D"}]}}, {"referenceToLCIAMethodDataSet": {"shortDescription": [{"value": "Auftreten von Krankheiten aufgrund von Feinstaubemissionen (PM)", "lang": "de"}, {"value": "Incidence of disease due to PM emissions (PM)", "lang": "en"}], "type": "LCIA method data set", "refObjectId": "b5c602c6-def3-11e6-bf01-fe55135034f3", "uri": "../lciamethods/b5c602c6-def3-11e6-bf01-fe55135034f3.xml"}, "other": {"anies": [{"name": "referenceToUnitGroupDataSet", "value": {"shortDescription": [{"value": "Krankheitsfälle", "lang": "de"}], "type": "unit group data set", "refObjectId": "3883559b-648f-4afc-8ba2-0bd24f3affa3", "uri": "../unitgroups/3883559b-648f-4afc-8ba2-0bd24f3affa3.xml"}}, {"value": "1.40915414112104E-05", "module": "A1-A3"}, {"value": "3.01632330763866E-08", "module": "A5"}, {"module": "B1"}, {"value": "0", "module": "C1"}, {"value": "6.85508049151704E-07", "module": "C2"}, {"value": "2.64891858805102E-06", "module": "C3"}, {"value": "0", "module": "C4"}, {"value": "-1.84340445952404E-06", "module": "D"}]}}, {"referenceToLCIAMethodDataSet": {"shortDescription": [{"value": "Wirkung durch Exposition des Menschen mit U235 (IR)", "lang": "de"}, {"value": "Human exposure efficiency relative to U235 (IR)", "lang": "en"}], "type": "LCIA method data set", "refObjectId": "b5c632be-def3-11e6-bf01-fe55135034f3", "uri": "../lciamethods/b5c632be-def3-11e6-bf01-fe55135034f3.xml"}, "other": {"anies": [{"name": "referenceToUnitGroupDataSet", "value": {"shortDescription": [{"value": "kBq U235-Äq.", "lang": "de"}], "type": "unit group data set", "refObjectId": "456b05bf-1415-44a9-9993-02452f554c09", "uri": "../unitgroups/456b05bf-1415-44a9-9993-02452f554c09.xml"}}, {"value": "13.7532841892737", "module": "A1-A3"}, {"value": "0.00195002432712424", "module": "A5"}, {"module": "B1"}, {"value": "0", "module": "C1"}, {"value": "0.0664876557169804", "module": "C2"}, {"value": "0.142492958291575", "module": "C3"}, {"value": "0", "module": "C4"}, {"value": "-8.74941394929715", "module": "D"}]}}, {"referenceToLCIAMethodDataSet": {"shortDescription": [{"value": "Toxizitätsvergleichseinheit für Ökosysteme (ETP-fw)", "lang": "de"}, {"value": "Comparative toxic unit for ecosystems (ETP-fw)", "lang": "en"}], "type": "LCIA method data set", "refObjectId": "ee1082d1-b0f7-43ca-a1f0-21e2a4a74511", "uri": "../lciamethods/ee1082d1-b0f7-43ca-a1f0-21e2a4a74511.xml"}, "other": {"anies": [{"name": "referenceToUnitGroupDataSet", "value": {"shortDescription": [{"value": "CTUe", "lang": "de"}], "type": "unit group data set", "refObjectId": "aa959ded-f1eb-4efb-9c5c-2d60be36b3e6", "uri": "../unitgroups/aa959ded-f1eb-4efb-9c5c-2d60be36b3e6.xml"}}, {"value": "1465.66431058344", "module": "A1-A3"}, {"value": "2.51090455819385", "module": "A5"}, {"module": "B1"}, {"value": "0", "module": "C1"}, {"value": "69.4989642655307", "module": "C2"}, {"value": "199.829268262195", "module": "C3"}, {"value": "0", "module": "C4"}, {"value": "-302.257886565611", "module": "D"}]}}, {"referenceToLCIAMethodDataSet": {"shortDescription": [{"value": "Toxizitätsvergleichseinheit für Menschen (krebserregend) (HTP-c)", "lang": "de"}, {"value": "Comparative toxic unit for humans (carcinogenic) (HTP-c)", "lang": "en"}], "type": "LCIA method data set", "refObjectId": "2299222a-bbd8-474f-9d4f-4dd1f18aea7c", "uri": "../lciamethods/2299222a-bbd8-474f-9d4f-4dd1f18aea7c.xml"}, "other": {"anies": [{"name": "referenceToUnitGroupDataSet", "value": {"shortDescription": [{"value": "CTUh", "lang": "de"}], "type": "unit group data set", "refObjectId": "d4c9523e-2d7e-49fd-8469-998f547d3a70", "uri": "../unitgroups/d4c9523e-2d7e-49fd-8469-998f547d3a70.xml"}}, {"value": "1.81155523266214E-07", "module": "A1-A3"}, {"value": "5.08725560059303E-10", "module": "A5"}, {"module": "B1"}, {"value": "0", "module": "C1"}, {"value": "4.21106394670079E-09", "module": "C2"}, {"value": "2.9914685088108E-08", "module": "C3"}, {"value": "0", "module": "C4"}, {"value": "-5.48773628871741E-08", "module": "D"}]}}, {"referenceToLCIAMethodDataSet": {"shortDescription": [{"value": "Toxizitätsvergleichseinheit für Menschen (nicht krebserregend) (HTP-nc)", "lang": "de"}, {"value": "Comparative toxic unit for humans (noncarcinogenic) (HTP-nc)", "lang": "en"}], "type": "LCIA method data set", "refObjectId": "3af763a5-b7a1-48c9-9cee-1f223481fcef", "uri": "../lciamethods/3af763a5-b7a1-48c9-9cee-1f223481fcef.xml"}, "other": {"anies": [{"name": "referenceToUnitGroupDataSet", "value": {"shortDescription": [{"value": "CTUh", "lang": "de"}], "type": "unit group data set", "refObjectId": "d4c9523e-2d7e-49fd-8469-998f547d3a70", "uri": "../unitgroups/d4c9523e-2d7e-49fd-8469-998f547d3a70.xml"}}, {"value": "6.28528784436845E-06", "module": "A1-A3"}, {"value": "2.44519420040999E-08", "module": "A5"}, {"module": "B1"}, {"value": "0", "module": "C1"}, {"value": "1.18554849649947E-07", "module": "C2"}, {"value": "1.03004070852602E-06", "module": "C3"}, {"value": "0", "module": "C4"}, {"value": "-1.44838949683235E-06", "module": "D"}]}}, {"referenceToLCIAMethodDataSet": {"shortDescription": [{"value": "Bodenqualitätsindex (SQP)", "lang": "de"}, {"value": "Soil quality index (SQP)", "lang": "en"}], "type": "LCIA method data set", "refObjectId": "b2ad6890-c78d-11e6-9d9d-cec0c932ce01", "uri": "../lciamethods/b2ad6890-c78d-11e6-9d9d-cec0c932ce01.xml"}, "other": {"anies": [{"name": "referenceToUnitGroupDataSet", "value": {"shortDescription": [{"value": "SQP", "lang": "de"}], "type": "unit group data set", "refObjectId": "f130951c-e67f-4f7f-8dd4-665de3974e18", "uri": "../unitgroups/f130951c-e67f-4f7f-8dd4-665de3974e18.xml"}}, {"value": "44057.7488905894", "module": "A1-A3"}, {"value": "1.39920791536116", "module": "A5"}, {"module": "B1"}, {"value": "0", "module": "C1"}, {"value": "79.2391882629074", "module": "C2"}, {"value": "264.059534957954", "module": "C3"}, {"value": "0", "module": "C4"}, {"value": "-348.817296408453", "module": "D"}]}}]}, "otherAttributes": {"{http://www.indata.network/EPD/2019}epd-version": "1.2"}, "version": "1.1", "locations": "../ILCDLocations.xml"}