{"processInformation": {"dataSetInformation": {"UUID": "d712008c-140f-4811-bee0-219cb6034244", "name": {"baseName": [{"value": "Stehfalzsystem für Dach und Fassade aus Aluminium", "lang": "de"}, {"value": "Standing Seam System for Aluminium Roofs and Façades", "lang": "en"}], "functionalUnitFlowProperties": [{"lang": "de"}]}, "classificationInformation": {"classification": [{"class": [{"value": "Komposite", "level": 0, "classId": "10"}, {"value": "Systembauteile", "level": 1, "classId": "10.1"}, {"value": "Aussenwände", "level": 2, "classId": "10.1.03"}], "name": "OEKOBAU.DAT"}, {"class": [{"value": "02 Bauprodukte", "level": 0}, {"value": "Bedachungen", "level": 1}, {"value": "Bedachungs- und Fassadensysteme aus Aluminium", "level": 2}], "name": "IBUCategories"}]}, "generalComment": [{"value": "Das BEMO Stehfalzsystem ist ein Dach- und Fassadensystem aus Aluminium. Die Stehfalzprofile werden werkseitig oder durch mobiles Rollformen, direkt vor Ort auf der Baustelle gefertigt.\nGrundstzlich kann das System in Breiten zwischen 80 mm und 600 mm hergestellt werden. Des Weiteren gibt es verschiedene Hhen und Ausfhrungen, je nachdem, was architektonisch und statisch gefordert wird. Neben den verschiedenen Breiten und Hhen, knnen die Profile auch konvex oder konkav bombiert werden.\nDarber hinaus gibt es die Mglichkeit konische und Freiform-Profile zu fertigen, die ebenfalls bombiert werden knnen. Die Oberflchen und Beschichtungen sind vielfltig. Die Aluminiumprofile knnen natur blank oder stucciert ausgefhrt werden. Hiermit wird nur die blanke Variante betrachtet. Das deklarierte System beinhaltet den wrmebrckenfreien GFK-Halter und das Stehfalzprofil.", "lang": "de"}, {"value": "The BEMO standing seam system is a roof and facade system made of aluminium. The standing seam profiles are manufactured at the factory or through mobile roll forming directly at the construction site.\nAs a general rule, the system can be produced in widths between 80 mm and 600 mm. Furthermore, various heights and designs are possible, depending on the specific architectonic and structural requirements. In addition to the various widths and heights, the profiles may also be raised in a convex or concave arrangement.\nThere is also the option of producing conical and free-form profiles which can also be raised. There are various surfaces and coatings. The aluminium profiles are available in natural sheer or stucco. Only the sheer version is examined here. The declared system includes the thermal bridge free GFRP clip and the standing seam profile. For putting the product on the market in the EU/EFTA (with the exception of Switzerland), Regulation (EU) No. 305/2011(CPR) applies. The product requires a Declaration of Performance taking into account ETA-15/0351 dated 21/06/2019, BEMO flat roof aluminium standingseam profile system, roof and wall systems with hidden fastenings and/or the general approval for use by the construction supervising authority Z-14.1-182 dated 02/04/2022 and the CE marking.", "lang": "en"}]}, "quantitativeReference": {"referenceToReferenceFlow": [0]}, "time": {"referenceYear": 2024, "dataSetValidUntil": 2029, "other": {"anies": [{"name": "publicationDateOfEPD", "value": 1718755200000}]}}, "geography": {"locationOfOperationSupplyOrProduction": {"location": "DE"}}, "technology": {"technologyDescriptionAndIncludedProcesses": [{"value": "Die Stehfalzprofile werden in Deutschland im Werk Ilshofen produziert. Die Komponente GFK-Halter wird extern zugekauft und im Bemo Werk kommissioniert und projektbezogen ausgeliefert.  \nTechnische Daten: \nDie deklarierte Einheit bezieht sich auf 1m Stehfalzsystem N65-305 mit Thermohalter 245/80 bestehend aus geraden Stehfalzprofiltafeln aus Aluminium und den dazugehrigen Haltern. \nDeklarierte Einheit: \nDie deklarierte Einheit bezieht sich auf 1m reprsentatives Stehfalzsystem BEMO N65-305 in 1,00 mm Dicke mit Thermohalter 245/80. Die in dieser EPD bilanzierte Aluminiumkomponente ist diejenige mit dem hchsten Gewicht/m aus allen 3 Typen, die von dieser EPD abgedeckt werden (N50, VF65 und N65). Die Ergebnisse der kobilanz gelten fr alle 3 genannten Produktvarianten mit einem Gewicht unter 4,31 kg Aluminium/m und mit einer Materialdicke zwischen 0,8 und 1,0 mm.\nFr die zweite Komponente gibt es insgesamt 7 Halteroptionen mit unterschiedlichen Gewichten, fr alle 7 Produktvarianten (schwerste Aluminiumkomponente mit allen 7 mglichen Haltertypen) wurden Ergebnisse berechnet.\nFr die deklarierte Einheit wurde die Variante mit dem hchsten Gewicht/m (0,47 kg/m) bilanziert. \nDie Schrauben fr die Montage des Produktes werden ebenfalls deklariert.", "lang": "de"}, {"value": "The aluminium profile is produced in the factory in Ilshofen in Germany. The GFRP clip component is purchased from a third party, picked and packed in the factory and delivered on a project-specific basis. \nTechnical data: \nThe declared unit refers to 1m standing seam system N65-305 with thermo clip 245/80 comprising straight standing seam profile panels made of aluminium and their related clips. \nDeclared unit: \nThe declared unit refers to a 1m2 representative standing seam system BEMO N65-305 in 1.00 mm thickness with thermo clip 245/80. The aluminium component assessed in this EPD is the one with the highest weight/m2 of all 3 types covered by this EPD (N50, VF65 and N65). The results of the life cycle assessment for all 3 named product versions weighing under 4.31 kg aluminium/m2 and with a material thickness between\n0.8 and 1.0 mm.\nFor the second component, there is a total of 7 clip options with different weights. Results were calculated for all 7 product versions (heaviest aluminium component with all 7 possible clip types).\nFor the declared unit, the version with the highest weight/m2 (0.47 kg/m2)was assessed.\nThe screws for the product assembly were also included in the declaration.", "lang": "en"}], "technologicalApplicability": [{"value": "Die kraftschlssig verfalzten und selbstragenden Stehfalzprofile werden im Dach und in der Fassade eingesetzt. Dabei werden die Profile auf Halter montiert und miteinander verbrdelt/verfalzt. Die Stehfalzprofile knnen im Dach ab einer Neigung von 1,5 Grad eingesetzt werden. Die Ausfhrung im Dach wie auch im Wandbereich (Fassade) kann hinterlftet, also als Kaltdach oder als gedmmte Konstruktion ausgefhrt werden.", "lang": "de"}, {"value": "The form-fit interlocked and self-supporting standing steel profiles are inserted into the roof and facade. Here, the profiles are fitted on clips and crimped/interlocked together. The standing seam profiles may be used on roofs with a pitch of 1.5 degrees or above. Both roof and wall (facade) versions can be ventilated, i.e. with a cold roof design or as an insulated structure.", "lang": "en"}]}}, "modellingAndValidation": {"LCIMethodAndAllocation": {"typeOfDataSet": "EPD", "referenceToLCAMethodDetails": [{"shortDescription": [{"value": "Bedachungs- und Fassadensysteme aus Aluminium.pdf", "lang": "de"}], "type": "source data set", "refObjectId": "21347176-4f7d-490b-bbf4-da0225303f14"}], "other": {"anies": [{"name": "subType", "value": "specific dataset"}]}}, "dataSourcesTreatmentAndRepresentativeness": {"referenceToDataSource": [{"shortDescription": [{"value": "GaBi Database (all versions)", "lang": "de"}], "type": "source data set", "refObjectId": "28d74cc0-db8b-4d7e-bc44-5f6d56ce0c4a"}, {"shortDescription": [{"value": "GaBi Database Edition 2022, CUP 2022.02", "lang": "de"}], "type": "source data set", "refObjectId": "94f442cb-662e-43ea-a792-4b0a35132e93"}], "useAdviceForDataSet": [{"value": "Gültigkeitsbereich: \nDie vorliegende EPD bezieht sich auf Herstellung, Transport und Entsorgung von einem reprsentativen Produkt mit den hchsten Umweltwirkungen (Worst-Case) fr eine Spanne von Produkten von BEMO. Die Ergebnisse der EPD sind gltig fr die Produktfamilien Typ N65, N50, VF65 in Dicken zwischen 0,8 mm und 1,0 mm, montiert mit dem Thermohalter Typ 245/80. Bei Verwendung anderer Haltertypen (65/80, 85/80, 125/80, 165/80, 205/80 oder 225/80) knnen die Umweltwirkungen mit Hilfe der Umrechnungstabellen berechnet werden. Die Produkte mit einer identischen Bezeichnung, aber mit einer Aluminiumstrke ber 1,0 mm werden von dieser EPD nicht abgedeckt. \nDie gesammelten Produktionsdaten beziehen sich auf das Jahr 2022. Die Herstellung der Stehfalzprofile aus Aluminium erfolgt im Bemo Werk in Ilshofen-Eckartshausen, Deutschland. \nSystemgrenze: \nDie Lebenszyklusanalyse fr das BEMO Stehfalzsystem umfasst die Lebenswegabschnitte \"von der Wiege bis Werkstor mit Optionen\" (cradle to gate with options). Bercksichtigt werden die Module A1-A3 als zusammengefasstes Modul fr die Herstellungsphase, A4-A5 (Errichtungsphase), C1-C4 (Entsorgungsphase) und D(Potenziale am Lebensende und Lasten auerhalb der Systemgrenze). \n\nIm Einzelnen wurden folgende Prozesse in das Informationsmodul A1-A3 der Herstellung des Stehfalzsystems einbezogen: \n- Bereitstellungsprozesse von Rohmaterial (Aluminium und glasfaserverstrkter Kunststoff) (A1) \n- Transporte der Roh-, Hilfs- und Betriebsstoffe zum Werk (A2) \n- Herstellungsprozesse fr das Systemprodukt im Werk, inkl. der energetischen Aufwendungen (Strom und Entsorgung von anfallenden Reststoffen (A3) \n- Herstellung von Verpackungsmaterialien (A3) \n- Transport vom Werkstor bis zur Baustelle (A4)\n- beim Einbau in das Gebude werden die Montageschrauben ebenfalls bercksichtigt. Der Dieselverbrauch fr den Transportkran bis aufs Dach, sowie der Energieverbrauch vom Akkuschauber wurden nicht herangezogen (A5). Hier kommt eine Unterschtzung der in Modul A5 auftretenden Umweltauswirkungen vor. \n- die Umweltlasten fr die Entsorgung der Verpackung (A5)\n- Rckbau und Abriss aus dem Gebude (C1) mithilfe eines Dieselbaggers, ohne Bercksichtigung des Diesels fr den Kran fr die Demontage. Es handelt sich hiermit um eine wesentliche Unterschtzung der in Modul C1 tatschlich auftretenden Umweltauswirkungen.\n- der Transport in einen Recyclinghof (C2)\n- Abfallbewirtschaftung zum Recycling des Aluminiums und thermische Behandlung des Halters (C3)\n- Deponiebetrieb fr das nicht brennbare Material aus dem Halter (C4) sowie fr das nicht gesammelte Aluminium (Verlust 5%)\n- Behandlung und Potenziale am Lebensende fr das in Modul D recycelte Aluminium (Recyclingrate 95%)", "lang": "de"}, {"value": "Scope: \nThis EPD refers to the manufacture, transport and disposal of a\nrepresentative product with the highest environmental impacts (worst case) for a range of BEMO products. The findings of the EPD are applicable to the product family types \nN65, N50, VF65 in thicknesses between 0.8 mm and 1.0 mm, fitted with thermo clip type 245/80. When using older clip types (65/80, 85/80, 125/80, 165/80, 205/80 or 225/80), the environmental impacts may be calculated using the conversion tables. Products with an identical designation but which have an aluminium thickness greater than 1.0 mm\nare not covered by this EPD.\nThe collected production data is for the year 2022. The aluminium standing seam profiles are manufactured in the Bemo factory in Ilshofen-Eckartshausen, Germany.\nThe owner of the declaration shall be liable for the underlying information and evidence; any liability of the IBU in relation to manufacturer information, LCA data and evidence is excluded.\n\nThe EPD was prepared in accordance with the requirements of\nEN 15804+A2. In the following, the standard is referred to in simplified form as EN 15804. \nSystem boundary: \nThe life cycle analysis for the BEMO standing seam system includes the stages \"cradle to gate with options\". Consideration is given to Modules A1-A3 as a combined module for the product stage, A4-A5 (construction stage), C1-C4 (end of life stage) and D (end-of-life potentials and loads beyond the system boundaries).\n\nIn particular, the following processes were included in information module A1-A3 for the production of the standing seam system:\n- Raw material supply (aluminium and glass-fibre reinforced plastic) (A1)\n- Transport of the raw and auxiliary materials and consumables to the factory (A2)\n- Production processes for the system product in the factory, including the energy costs (power and disposal of residual substances) (A3)\n- Production of packaging materials (A3)\n- Transport from the factory gate to the construction site (A4)\n- When installed in the building, the assembly screws are also considered. The diesel consumption for the transport crane to the roof, as well as the energy consumption, are not included.\n- Environmental impacts for the disposal of the packaging (A5).\n- De-construction and demolition from the building (C1) using a diesel excavator, without taking into account the\ndiesel used by the crane for disassembly.\n- Transportation to a recycling centre (C2)\n- Waste processing for recycling the aluminium and thermal treatment of the clip (C3)\n- Landfill operation for the non-flammable material from the clip (C4) and for the aluminium not collected (loss 5%)\n- Treatment and potentials at end of life for the aluminium recycled in Module D (recycling rate 95%)", "lang": "en"}], "other": {"anies": [{"name": "referenceToOriginalEPD", "value": {"shortDescription": {"value": "Stehfalzsystem für Dach und Fassade aus Aluminium.pdf", "defaultValue": "Stehfalzsystem für Dach und Fassade aus Aluminium.pdf", "lstrings": [{"lang": "de", "value": "Stehfalzsystem für Dach und Fassade aus Aluminium.pdf"}]}, "type": "source data set", "uuid": {"uuid": "959df800-4e80-40fc-ad0c-09756338fa42"}, "refObjectId": "959df800-4e80-40fc-ad0c-09756338fa42", "resourceURLs": ["https://oekobaudat.de/OEKOBAU.DAT/resource/sources/959df800-4e80-40fc-ad0c-09756338fa42/Stehfalzsystem_fuer_Dach_und_Fassade_aus_Aluminium_16985.pdf?version=00.01.000"]}}]}}, "validation": {"review": [{"referenceToNameOfReviewerAndInstitution": [{"shortDescription": [{"value": "Institut Bauen und Umwelt e. V.", "lang": "de"}], "type": "contact data set", "refObjectId": "d111dbec-b024-4be5-86c5-752d6eb2cf95", "uri": "../contacts/.xml"}], "type": "Accredited third party review"}]}, "complianceDeclarations": {"compliance": [{"referenceToComplianceSystem": {"shortDescription": [{"value": "DIN EN 15804+A2", "lang": "de"}], "type": "source data set", "refObjectId": "c0016b33-8cf7-415c-ac6e-deba0d21440d", "uri": "../sources/c0016b33-8cf7-415c-ac6e-deba0d21440d.xml"}}, {"referenceToComplianceSystem": {"shortDescription": [{"value": "ISO 14025", "lang": "de"}], "type": "source data set", "refObjectId": "4f2eb655-6e44-4874-a95a-e28f5442cd4d", "uri": "../sources/4f2eb655-6e44-4874-a95a-e28f5442cd4d.xml"}}]}}, "administrativeInformation": {"commissionerAndGoal": {"referenceToCommissioner": [{"shortDescription": [{"value": "BEMO SYSTEMS GmbH", "lang": "de"}], "type": "contact data set", "refObjectId": "e3540c1e-8040-47d9-8f92-8a5d8040bf30", "uri": "../contacts/e3540c1e-8040-47d9-8f92-8a5d8040bf30.xml"}]}, "dataGenerator": {"referenceToPersonOrEntityGeneratingTheDataSet": [{"shortDescription": [{"value": "Lindner Group", "lang": "de"}], "type": "contact data set", "refObjectId": "35a13c35-3b24-4ac9-be18-ee4fd3501146", "uri": "../contacts/35a13c35-3b24-4ac9-be18-ee4fd3501146.xml"}]}, "dataEntryBy": {"timeStamp": 1718755200000, "referenceToDataSetFormat": [{"shortDescription": [{"value": "ILCD Format", "lang": "de"}], "type": "source data set", "refObjectId": "a97a0155-0234-4b87-b4ce-a45da52f2a40", "uri": "../sources/a97a0155-0234-4b87-b4ce-a45da52f2a40.xml"}, {"shortDescription": [{"value": "EPD-Datenformaterweiterungen v1.2", "lang": "de"}, {"value": "EPD Data Format Extensions v1.2", "lang": "en"}], "type": "source data set", "refObjectId": "a29449fd-aa2f-4de8-b5d7-4b06b43c6fde", "uri": "../sources/a29449fd-aa2f-4de8-b5d7-4b06b43c6fde.xml"}]}, "publicationAndOwnership": {"dataSetVersion": "00.01.200", "referenceToRegistrationAuthority": {"shortDescription": [{"value": "Institut Bauen und Umwelt e. V.", "lang": "de"}], "type": "contact data set", "refObjectId": "d111dbec-b024-4be5-86c5-752d6eb2cf95", "uri": "../contacts/d111dbec-b024-4be5-86c5-752d6eb2cf95.xml"}, "registrationNumber": "EPD-BEM-20230118-IBC1-DE", "referenceToOwnershipOfDataSet": {"shortDescription": [{"value": "BEMO SYSTEMS GmbH", "lang": "de"}], "type": "contact data set", "refObjectId": "e3540c1e-8040-47d9-8f92-8a5d8040bf30", "uri": "../contacts/e3540c1e-8040-47d9-8f92-8a5d8040bf30.xml"}, "copyright": true, "licenseType": "Free of charge for all users and uses", "accessRestrictions": [{"value": "None", "lang": "en"}], "other": {"anies": [{"name": "referenceToPublisher", "value": {"shortDescription": [{"value": "Institut Bauen und Umwelt e. V.", "lang": "de"}], "type": "contact data set", "refObjectId": "d111dbec-b024-4be5-86c5-752d6eb2cf95", "uri": "../contacts/d111dbec-b024-4be5-86c5-752d6eb2cf95.xml"}}]}}}, "exchanges": {"exchange": [{"dataSetInternalID": 0, "referenceToFlowDataSet": {"shortDescription": [{"value": "Stehfalzsystem ()", "lang": "de"}], "type": "flow data set", "refObjectId": "ca0ef97f-c5ff-4551-acc9-5801fcbb26a1", "uri": "../flows/ca0ef97f-c5ff-4551-acc9-5801fcbb26a1.xml"}, "meanAmount": 1.0, "referencesToDataSource": {}, "referenceFlow": true, "resolvedFlowVersion": "00.01.100", "resultingflowAmount": 1.0, "flowProperties": [{"name": [{"lang": "de", "value": "Fläche"}, {"lang": "en", "value": "Area"}], "uuid": "93a60a56-a3c8-19da-a746-0800200c9a66", "referenceFlowProperty": true, "meanValue": 1.0, "referenceUnit": "qm", "unitGroupUUID": "c20a03d7-bd90-4569-bc94-66cfd364dfc8"}], "materialProperties": [{"name": "grammage", "value": "4.205", "unit": "kg/m^2", "unitDescription": "kilograms per square meter"}, {"name": "layer thickness", "value": "0.001", "unit": "m", "unitDescription": "meters"}], "typeOfFlow": "Product flow", "classification": {"classHierarchy": "Komposite / Systembauteile / Aussenwände", "name": "OEKOBAU.DAT"}}, {"dataSetInternalID": 1, "referenceToFlowDataSet": {"shortDescription": [{"value": "Erneuerbare Primärenergie als Energieträger (PERE)", "lang": "de"}, {"value": "Renewable primary energy as energy carrier (PERE)", "lang": "en"}], "type": "flow data set", "refObjectId": "20f32be5-0398-4288-9b6d-accddd195317", "uri": "../flows/20f32be5-0398-4288-9b6d-accddd195317.xml"}, "exchange direction": "INPUT", "other": {"anies": [{"name": "referenceToUnitGroupDataSet", "value": {"shortDescription": [{"value": "MJ", "lang": "de"}], "type": "unit group data set", "refObjectId": "93a60a57-a3c8-11da-a746-0800200c9a66", "uri": "../unitgroups/93a60a57-a3c8-11da-a746-0800200c9a66.xml"}}, {"value": "138.301669637203", "module": "A1-A3"}, {"value": "0.190236445918314", "module": "A4"}, {"value": "9.64", "module": "A5"}, {"value": "0.00294745936224311", "module": "C1"}, {"value": "0.0421908941998476", "module": "C2"}, {"value": "0.135130318779929", "module": "C3"}, {"value": "0.0174", "module": "C4"}, {"value": "-116.320446640178", "module": "D"}]}, "resolvedFlowVersion": "38.00.000", "flowProperties": [], "typeOfFlow": "Other flow", "classification": {"classHierarchy": "Quantities", "name": "GaBiCategories"}}, {"dataSetInternalID": 2, "referenceToFlowDataSet": {"shortDescription": [{"value": "Erneuerbare Primärenergie zur stofflichen Nutzung (PERM)", "lang": "de"}, {"value": "Renewable primary energy resources as material utilization (PERM)", "lang": "en"}], "type": "flow data set", "refObjectId": "fb3ec0de-548d-4508-aea5-00b73bf6f702", "uri": "../flows/fb3ec0de-548d-4508-aea5-00b73bf6f702.xml"}, "exchange direction": "INPUT", "other": {"anies": [{"name": "referenceToUnitGroupDataSet", "value": {"shortDescription": [{"value": "MJ", "lang": "de"}], "type": "unit group data set", "refObjectId": "93a60a57-a3c8-11da-a746-0800200c9a66", "uri": "../unitgroups/93a60a57-a3c8-11da-a746-0800200c9a66.xml"}}, {"value": "9.200736", "module": "A1-A3"}, {"value": "0", "module": "A4"}, {"value": "-9.200736", "module": "A5"}, {"value": "0", "module": "C1"}, {"value": "0", "module": "C2"}, {"value": "0", "module": "C3"}, {"value": "0", "module": "C4"}, {"value": "0", "module": "D"}]}, "resolvedFlowVersion": "38.00.000", "flowProperties": [], "typeOfFlow": "Other flow", "classification": {"classHierarchy": "Quantities", "name": "GaBiCategories"}}, {"dataSetInternalID": 3, "referenceToFlowDataSet": {"shortDescription": [{"value": "Total erneuerbare Primärenergie (PERT)", "lang": "de"}, {"value": "Total use of renewable primary energy resources (PERT)", "lang": "en"}], "type": "flow data set", "refObjectId": "53f97275-fa8a-4cdd-9024-65936002acd0", "uri": "../flows/53f97275-fa8a-4cdd-9024-65936002acd0.xml"}, "exchange direction": "INPUT", "other": {"anies": [{"name": "referenceToUnitGroupDataSet", "value": {"shortDescription": [{"value": "MJ", "lang": "de"}], "type": "unit group data set", "refObjectId": "93a60a57-a3c8-11da-a746-0800200c9a66", "uri": "../unitgroups/93a60a57-a3c8-11da-a746-0800200c9a66.xml"}}, {"value": "147.502405637203", "module": "A1-A3"}, {"value": "0.190236445918314", "module": "A4"}, {"value": "0.44", "module": "A5"}, {"value": "0.00294745936224311", "module": "C1"}, {"value": "0.0421908941998476", "module": "C2"}, {"value": "0.135130318779929", "module": "C3"}, {"value": "0.0174", "module": "C4"}, {"value": "-116.320446640178", "module": "D"}]}, "resolvedFlowVersion": "38.00.000", "flowProperties": [], "typeOfFlow": "Other flow", "classification": {"classHierarchy": "Quantities / Environmental quantities / EPD EN 15804 / LCI indicators", "name": "GaBiCategories"}}, {"dataSetInternalID": 4, "referenceToFlowDataSet": {"shortDescription": [{"value": "Nicht-erneuerbare Primärenergie als Energieträger (PENRE)", "lang": "de"}, {"value": "Non renewable primary energy as energy carrier (PENRE)", "lang": "en"}], "type": "flow data set", "refObjectId": "ac857178-2b45-46ec-892a-a9a4332f0372", "uri": "../flows/ac857178-2b45-46ec-892a-a9a4332f0372.xml"}, "exchange direction": "INPUT", "other": {"anies": [{"name": "referenceToUnitGroupDataSet", "value": {"shortDescription": [{"value": "MJ", "lang": "de"}], "type": "unit group data set", "refObjectId": "93a60a57-a3c8-11da-a746-0800200c9a66", "uri": "../unitgroups/93a60a57-a3c8-11da-a746-0800200c9a66.xml"}}, {"value": "343.995481852325", "module": "A1-A3"}, {"value": "2.8427755603556", "module": "A4"}, {"value": "1.65", "module": "A5"}, {"value": "0.0440450062009879", "module": "C1"}, {"value": "0.630474577686217", "module": "C2"}, {"value": "8.36275918081948", "module": "C3"}, {"value": "0.181", "module": "C4"}, {"value": "-263.65925371425", "module": "D"}]}, "resolvedFlowVersion": "38.00.000", "flowProperties": [], "typeOfFlow": "Other flow", "classification": {"classHierarchy": "Quantities", "name": "GaBiCategories"}}, {"dataSetInternalID": 5, "referenceToFlowDataSet": {"shortDescription": [{"value": "Nicht-erneuerbare Primärenergie zur stofflichen Nutzung (PENRM)", "lang": "de"}, {"value": "Non renewable primary energy as material utilization (PENRM)", "lang": "en"}], "type": "flow data set", "refObjectId": "1421caa0-679d-4bf4-b282-0eb850ccae27", "uri": "../flows/1421caa0-679d-4bf4-b282-0eb850ccae27.xml"}, "exchange direction": "INPUT", "other": {"anies": [{"name": "referenceToUnitGroupDataSet", "value": {"shortDescription": [{"value": "MJ", "lang": "de"}], "type": "unit group data set", "refObjectId": "93a60a57-a3c8-11da-a746-0800200c9a66", "uri": "../unitgroups/93a60a57-a3c8-11da-a746-0800200c9a66.xml"}}, {"value": "7.9524", "module": "A1-A3"}, {"value": "0", "module": "A4"}, {"value": "0", "module": "A5"}, {"value": "0", "module": "C1"}, {"value": "0", "module": "C2"}, {"value": "-7.9524", "module": "C3"}, {"value": "0", "module": "C4"}, {"value": "0", "module": "D"}]}, "resolvedFlowVersion": "38.00.000", "flowProperties": [], "typeOfFlow": "Other flow", "classification": {"classHierarchy": "Quantities", "name": "GaBiCategories"}}, {"dataSetInternalID": 6, "referenceToFlowDataSet": {"shortDescription": [{"value": "Total nicht erneuerbare Primärenergie (PENRT)", "lang": "de"}, {"value": "Total use of non renewable primary energy resources (PENRT)", "lang": "en"}], "type": "flow data set", "refObjectId": "06159210-646b-4c8d-8583-da9b3b95a6c1", "uri": "../flows/06159210-646b-4c8d-8583-da9b3b95a6c1.xml"}, "exchange direction": "INPUT", "other": {"anies": [{"name": "referenceToUnitGroupDataSet", "value": {"shortDescription": [{"value": "MJ", "lang": "de"}], "type": "unit group data set", "refObjectId": "93a60a57-a3c8-11da-a746-0800200c9a66", "uri": "../unitgroups/93a60a57-a3c8-11da-a746-0800200c9a66.xml"}}, {"value": "351.947881852326", "module": "A1-A3"}, {"value": "2.8427755603556", "module": "A4"}, {"value": "1.65", "module": "A5"}, {"value": "0.0440450062009879", "module": "C1"}, {"value": "0.630474577686217", "module": "C2"}, {"value": "0.410359180819473", "module": "C3"}, {"value": "0.181", "module": "C4"}, {"value": "-263.65925371425", "module": "D"}]}, "resolvedFlowVersion": "38.00.000", "flowProperties": [], "typeOfFlow": "Other flow", "classification": {"classHierarchy": "Quantities / Environmental quantities / EPD EN 15804 / LCI indicators", "name": "GaBiCategories"}}, {"dataSetInternalID": 7, "referenceToFlowDataSet": {"shortDescription": [{"value": "Einsatz von Sekundärstoffen (SM)", "lang": "de"}, {"value": "Use of secondary material (SM)", "lang": "en"}], "type": "flow data set", "refObjectId": "c6a1f35f-2d09-4f54-8dfb-97e502e1ce92", "uri": "../flows/c6a1f35f-2d09-4f54-8dfb-97e502e1ce92.xml"}, "exchange direction": "INPUT", "other": {"anies": [{"name": "referenceToUnitGroupDataSet", "value": {"shortDescription": [{"value": "kg", "lang": "de"}], "type": "unit group data set", "refObjectId": "ad38d542-3fe9-439d-9b95-2f5f7752acaf", "uri": "../unitgroups/ad38d542-3fe9-439d-9b95-2f5f7752acaf.xml"}}, {"value": "1.73", "module": "A1-A3"}, {"value": "0", "module": "A4"}, {"value": "0.022", "module": "A5"}, {"value": "0", "module": "C1"}, {"value": "0", "module": "C2"}, {"value": "0", "module": "C3"}, {"value": "0", "module": "C4"}, {"value": "2.37", "module": "D"}]}, "resolvedFlowVersion": "38.00.000", "flowProperties": [], "typeOfFlow": "Other flow", "classification": {"classHierarchy": "Quantities / Environmental quantities / EPD EN 15804 / LCI indicators", "name": "GaBiCategories"}}, {"dataSetInternalID": 8, "referenceToFlowDataSet": {"shortDescription": [{"value": "Erneuerbare Sekundärbrennstoffe (RSF)", "lang": "de"}, {"value": "Use of renewable secondary fuels (RSF)", "lang": "en"}], "type": "flow data set", "refObjectId": "64333088-a55f-4aa2-9a31-c10b07816787", "uri": "../flows/64333088-a55f-4aa2-9a31-c10b07816787.xml"}, "exchange direction": "INPUT", "other": {"anies": [{"name": "referenceToUnitGroupDataSet", "value": {"shortDescription": [{"value": "MJ", "lang": "de"}], "type": "unit group data set", "refObjectId": "93a60a57-a3c8-11da-a746-0800200c9a66", "uri": "../unitgroups/93a60a57-a3c8-11da-a746-0800200c9a66.xml"}}, {"value": "0", "module": "A1-A3"}, {"value": "0", "module": "A4"}, {"value": "0", "module": "A5"}, {"value": "0", "module": "C1"}, {"value": "0", "module": "C2"}, {"value": "0", "module": "C3"}, {"value": "0", "module": "C4"}, {"value": "0", "module": "D"}]}, "resolvedFlowVersion": "38.00.000", "flowProperties": [], "typeOfFlow": "Other flow", "classification": {"classHierarchy": "Quantities / Environmental quantities / EPD EN 15804 / LCI indicators", "name": "GaBiCategories"}}, {"dataSetInternalID": 9, "referenceToFlowDataSet": {"shortDescription": [{"value": "Nicht erneuerbare Sekundärbrennstoffe (NRSF)", "lang": "de"}, {"value": "Use of non renewable secondary fuels (NRSF)", "lang": "en"}], "type": "flow data set", "refObjectId": "89def144-d39a-4287-b86f-efde453ddcb2", "uri": "../flows/89def144-d39a-4287-b86f-efde453ddcb2.xml"}, "exchange direction": "INPUT", "other": {"anies": [{"name": "referenceToUnitGroupDataSet", "value": {"shortDescription": [{"value": "MJ", "lang": "de"}], "type": "unit group data set", "refObjectId": "93a60a57-a3c8-11da-a746-0800200c9a66", "uri": "../unitgroups/93a60a57-a3c8-11da-a746-0800200c9a66.xml"}}, {"value": "0", "module": "A1-A3"}, {"value": "0", "module": "A4"}, {"value": "0", "module": "A5"}, {"value": "0", "module": "C1"}, {"value": "0", "module": "C2"}, {"value": "0", "module": "C3"}, {"value": "0", "module": "C4"}, {"value": "0", "module": "D"}]}, "resolvedFlowVersion": "38.00.000", "flowProperties": [], "typeOfFlow": "Other flow", "classification": {"classHierarchy": "Quantities / Environmental quantities / EPD EN 15804 / LCI indicators", "name": "GaBiCategories"}}, {"dataSetInternalID": 10, "referenceToFlowDataSet": {"shortDescription": [{"value": "Einsatz von Süßwasserressourcen (FW)", "lang": "de"}, {"value": "Use of net fresh water (FW)", "lang": "en"}], "type": "flow data set", "refObjectId": "3cf952c8-f3a4-461d-8c96-96456ca62246", "uri": "../flows/3cf952c8-f3a4-461d-8c96-96456ca62246.xml"}, "exchange direction": "INPUT", "other": {"anies": [{"name": "referenceToUnitGroupDataSet", "value": {"shortDescription": [{"value": "m^3", "lang": "de"}], "type": "unit group data set", "refObjectId": "cd950537-0a98-4044-9ba7-9f9a68d0a504", "uri": "../unitgroups/cd950537-0a98-4044-9ba7-9f9a68d0a504.xml"}}, {"value": "0.338036303520242", "module": "A1-A3"}, {"value": "0.000169268732994722", "module": "A4"}, {"value": "0.0029", "module": "A5"}, {"value": "2.6225926866535E-06", "module": "C1"}, {"value": "3.75406466970531E-05", "module": "C2"}, {"value": "0.00181048024825234", "module": "C3"}, {"value": "9.24E-06", "module": "C4"}, {"value": "-0.288233115324033", "module": "D"}]}, "resolvedFlowVersion": "38.00.000", "flowProperties": [], "typeOfFlow": "Other flow", "classification": {"classHierarchy": "Quantities / Environmental quantities / EPD EN 15804 / LCI indicators", "name": "GaBiCategories"}}, {"dataSetInternalID": 11, "referenceToFlowDataSet": {"shortDescription": [{"value": "Gefährlicher Abfall zur Deponie (HWD)", "lang": "de"}, {"value": "Hazardous waste disposed (HWD)", "lang": "en"}], "type": "flow data set", "refObjectId": "430f9e0f-59b2-46a0-8e0d-55e0e84948fc", "uri": "../flows/430f9e0f-59b2-46a0-8e0d-55e0e84948fc.xml"}, "exchange direction": "OUTPUT", "other": {"anies": [{"name": "referenceToUnitGroupDataSet", "value": {"shortDescription": [{"value": "kg", "lang": "de"}], "type": "unit group data set", "refObjectId": "ad38d542-3fe9-439d-9b95-2f5f7752acaf", "uri": "../unitgroups/ad38d542-3fe9-439d-9b95-2f5f7752acaf.xml"}}, {"value": "3.64823883634335E-08", "module": "A1-A3"}, {"value": "4.7911287591212E-12", "module": "A4"}, {"value": "7E-12", "module": "A5"}, {"value": "7.42321338512E-14", "module": "C1"}, {"value": "1.0625829640485E-12", "module": "C2"}, {"value": "-7.8799650469023E-12", "module": "C3"}, {"value": "4.69E-10", "module": "C4"}, {"value": "-1.29454916660123E-08", "module": "D"}]}, "resolvedFlowVersion": "38.00.000", "flowProperties": [], "typeOfFlow": "Other flow", "classification": {"classHierarchy": "Quantities / Environmental quantities / EPD EN 15804 / LCI indicators", "name": "GaBiCategories"}}, {"dataSetInternalID": 12, "referenceToFlowDataSet": {"shortDescription": [{"value": "Entsorgter nicht gefährlicher Abfall (NHWD)", "lang": "de"}, {"value": "Non hazardous waste disposed (NHWD)", "lang": "en"}], "type": "flow data set", "refObjectId": "b29ef66b-e286-4afa-949f-62f1a7b4d7fa", "uri": "../flows/b29ef66b-e286-4afa-949f-62f1a7b4d7fa.xml"}, "exchange direction": "OUTPUT", "other": {"anies": [{"name": "referenceToUnitGroupDataSet", "value": {"shortDescription": [{"value": "kg", "lang": "de"}], "type": "unit group data set", "refObjectId": "ad38d542-3fe9-439d-9b95-2f5f7752acaf", "uri": "../unitgroups/ad38d542-3fe9-439d-9b95-2f5f7752acaf.xml"}}, {"value": "6.71100070153947", "module": "A1-A3"}, {"value": "0.0322", "module": "A4"}, {"value": "0.0322580802803304", "module": "A5"}, {"value": "6.59094169568717E-06", "module": "C1"}, {"value": "9.43448881169562E-05", "module": "C2"}, {"value": "0.0806157003612315", "module": "C3"}, {"value": "0.366", "module": "C4"}, {"value": "-5.7898733842449", "module": "D"}]}, "resolvedFlowVersion": "38.00.000", "flowProperties": [], "typeOfFlow": "Other flow", "classification": {"classHierarchy": "Quantities / Environmental quantities / EPD EN 15804 / LCI indicators", "name": "GaBiCategories"}}, {"dataSetInternalID": 13, "referenceToFlowDataSet": {"shortDescription": [{"value": "Entsorgter radioaktiver Abfall (RWD)", "lang": "de"}, {"value": "Radioactive waste disposed (RWD)", "lang": "en"}], "type": "flow data set", "refObjectId": "3449546e-52ad-4b39-b809-9fb77cea8ff6", "uri": "../flows/3449546e-52ad-4b39-b809-9fb77cea8ff6.xml"}, "exchange direction": "OUTPUT", "other": {"anies": [{"name": "referenceToUnitGroupDataSet", "value": {"shortDescription": [{"value": "kg", "lang": "de"}], "type": "unit group data set", "refObjectId": "ad38d542-3fe9-439d-9b95-2f5f7752acaf", "uri": "../unitgroups/ad38d542-3fe9-439d-9b95-2f5f7752acaf.xml"}}, {"value": "0.0195962507449624", "module": "A1-A3"}, {"value": "3.7413492551672E-06", "module": "A4"}, {"value": "5.45E-05", "module": "A5"}, {"value": "5.7967204109243E-08", "module": "C1"}, {"value": "8.29761457261549E-07", "module": "C2"}, {"value": "1.38132827157953E-05", "module": "C3"}, {"value": "2.09E-06", "module": "C4"}, {"value": "-0.0154291389414143", "module": "D"}]}, "resolvedFlowVersion": "38.00.000", "flowProperties": [], "typeOfFlow": "Other flow", "classification": {"classHierarchy": "Quantities / Environmental quantities / EPD EN 15804 / LCI indicators", "name": "GaBiCategories"}}, {"dataSetInternalID": 14, "referenceToFlowDataSet": {"shortDescription": [{"value": "Komponenten für die Wiederverwendung (CRU)", "lang": "de"}, {"value": "Components for re-use (CRU)", "lang": "en"}], "type": "flow data set", "refObjectId": "a2b32f97-3fc7-4af2-b209-525bc6426f33", "uri": "../flows/a2b32f97-3fc7-4af2-b209-525bc6426f33.xml"}, "exchange direction": "OUTPUT", "other": {"anies": [{"name": "referenceToUnitGroupDataSet", "value": {"shortDescription": [{"value": "kg", "lang": "de"}], "type": "unit group data set", "refObjectId": "ad38d542-3fe9-439d-9b95-2f5f7752acaf", "uri": "../unitgroups/ad38d542-3fe9-439d-9b95-2f5f7752acaf.xml"}}, {"value": "0", "module": "A1-A3"}, {"value": "0", "module": "A4"}, {"value": "0", "module": "A5"}, {"value": "0", "module": "C1"}, {"value": "0", "module": "C2"}, {"value": "0", "module": "C3"}, {"value": "0", "module": "C4"}, {"value": "0", "module": "D"}]}, "resolvedFlowVersion": "38.00.000", "flowProperties": [], "typeOfFlow": "Other flow", "classification": {"classHierarchy": "Quantities / Environmental quantities / EPD EN 15804 / LCI indicators", "name": "GaBiCategories"}}, {"dataSetInternalID": 15, "referenceToFlowDataSet": {"shortDescription": [{"value": "Stoffe zum Recycling (MFR)", "lang": "de"}, {"value": "Materials for recycling (MFR)", "lang": "en"}], "type": "flow data set", "refObjectId": "d7fe48a5-4103-49c8-9aae-b0b5dfdbd6ae", "uri": "../flows/d7fe48a5-4103-49c8-9aae-b0b5dfdbd6ae.xml"}, "exchange direction": "OUTPUT", "other": {"anies": [{"name": "referenceToUnitGroupDataSet", "value": {"shortDescription": [{"value": "kg", "lang": "de"}], "type": "unit group data set", "refObjectId": "ad38d542-3fe9-439d-9b95-2f5f7752acaf", "uri": "../unitgroups/ad38d542-3fe9-439d-9b95-2f5f7752acaf.xml"}}, {"value": "0.08", "module": "A1-A3"}, {"value": "0", "module": "A4"}, {"value": "0.011", "module": "A5"}, {"value": "0", "module": "C1"}, {"value": "0", "module": "C2"}, {"value": "4.0945", "module": "C3"}, {"value": "0", "module": "C4"}, {"value": "0", "module": "D"}]}, "resolvedFlowVersion": "38.00.000", "flowProperties": [], "typeOfFlow": "Other flow", "classification": {"classHierarchy": "Quantities / Environmental quantities / EPD EN 15804 / LCI indicators", "name": "GaBiCategories"}}, {"dataSetInternalID": 16, "referenceToFlowDataSet": {"shortDescription": [{"value": "Stoffe für die Energierückgewinnung (MER)", "lang": "de"}, {"value": "Materials for energy recovery (MER)", "lang": "en"}], "type": "flow data set", "refObjectId": "59a9181c-3aaf-46ee-8b13-2b3723b6e447", "uri": "../flows/59a9181c-3aaf-46ee-8b13-2b3723b6e447.xml"}, "exchange direction": "OUTPUT", "other": {"anies": [{"name": "referenceToUnitGroupDataSet", "value": {"shortDescription": [{"value": "kg", "lang": "de"}], "type": "unit group data set", "refObjectId": "ad38d542-3fe9-439d-9b95-2f5f7752acaf", "uri": "../unitgroups/ad38d542-3fe9-439d-9b95-2f5f7752acaf.xml"}}, {"value": "0", "module": "A1-A3"}, {"value": "0", "module": "A4"}, {"value": "0", "module": "A5"}, {"value": "0", "module": "C1"}, {"value": "0", "module": "C2"}, {"value": "0", "module": "C3"}, {"value": "0", "module": "C4"}, {"value": "0", "module": "D"}]}, "resolvedFlowVersion": "38.00.000", "flowProperties": [], "typeOfFlow": "Other flow", "classification": {"classHierarchy": "Quantities / Environmental quantities / EPD EN 15804 / LCI indicators", "name": "GaBiCategories"}}, {"dataSetInternalID": 17, "referenceToFlowDataSet": {"shortDescription": [{"value": "Exportierte elektrische Energie (EEE)", "lang": "de"}, {"value": "Exported electrical energy (EEE)", "lang": "en"}], "type": "flow data set", "refObjectId": "4da0c987-2b76-40d6-9e9e-82a017aaaf29", "uri": "../flows/4da0c987-2b76-40d6-9e9e-82a017aaaf29.xml"}, "exchange direction": "OUTPUT", "other": {"anies": [{"name": "referenceToUnitGroupDataSet", "value": {"shortDescription": [{"value": "MJ", "lang": "de"}], "type": "unit group data set", "refObjectId": "93a60a57-a3c8-11da-a746-0800200c9a66", "uri": "../unitgroups/93a60a57-a3c8-11da-a746-0800200c9a66.xml"}}, {"value": "0", "module": "A1-A3"}, {"value": "0", "module": "A4"}, {"value": "1.25150206366681", "module": "A5"}, {"value": "0", "module": "C1"}, {"value": "0", "module": "C2"}, {"value": "1.23287834761432", "module": "C3"}, {"value": "0", "module": "C4"}, {"value": "2.48438041128113", "module": "D"}]}, "resolvedFlowVersion": "38.00.000", "flowProperties": [], "typeOfFlow": "Other flow", "classification": {"classHierarchy": "Quantities / Environmental quantities / EPD EN 15804 / LCI indicators", "name": "GaBiCategories"}}, {"dataSetInternalID": 18, "referenceToFlowDataSet": {"shortDescription": [{"value": "Exportierte thermische Energie (EET)", "lang": "de"}, {"value": "Exported thermal energy (EET)", "lang": "en"}], "type": "flow data set", "refObjectId": "98daf38a-7a79-46d3-9a37-2b7bd0955810", "uri": "../flows/98daf38a-7a79-46d3-9a37-2b7bd0955810.xml"}, "exchange direction": "OUTPUT", "other": {"anies": [{"name": "referenceToUnitGroupDataSet", "value": {"shortDescription": [{"value": "MJ", "lang": "de"}], "type": "unit group data set", "refObjectId": "93a60a57-a3c8-11da-a746-0800200c9a66", "uri": "../unitgroups/93a60a57-a3c8-11da-a746-0800200c9a66.xml"}}, {"value": "0", "module": "A1-A3"}, {"value": "0", "module": "A4"}, {"value": "2.25543463139551", "module": "A5"}, {"value": "0", "module": "C1"}, {"value": "0", "module": "C2"}, {"value": "2.85654642798345", "module": "C3"}, {"value": "0", "module": "C4"}, {"value": "5.11198105937896", "module": "D"}]}, "resolvedFlowVersion": "38.00.000", "flowProperties": [], "typeOfFlow": "Other flow", "classification": {"classHierarchy": "Quantities / Environmental quantities / EPD EN 15804 / LCI indicators", "name": "GaBiCategories"}}]}, "LCIAResults": {"LCIAResult": [{"referenceToLCIAMethodDataSet": {"shortDescription": [{"value": "Globales Erwärmungspotenzial total (GWP-total)", "lang": "de"}, {"value": "Global Warming Potential total (GWP-total)", "lang": "en"}], "type": "LCIA method data set", "refObjectId": "6a37f984-a4b3-458a-a20a-64418c145fa2", "uri": "../lciamethods/6a37f984-a4b3-458a-a20a-64418c145fa2.xml"}, "other": {"anies": [{"name": "referenceToUnitGroupDataSet", "value": {"shortDescription": [{"value": "kg CO_(2)-Äq.", "lang": "de"}], "type": "unit group data set", "refObjectId": "1ebf3012-d0db-4de2-aefd-ef30cedb0be1", "uri": "../unitgroups/1ebf3012-d0db-4de2-aefd-ef30cedb0be1.xml"}}, {"value": "25.1975857834223", "module": "A1-A3"}, {"value": "0.20368713729239", "module": "A4"}, {"value": "1.17004576615056", "module": "A5"}, {"value": "0.00327240673611862", "module": "C1"}, {"value": "0.0461457477413632", "module": "C2"}, {"value": "0.806490020861692", "module": "C3"}, {"value": "0.0123", "module": "C4"}, {"value": "-20.1799272282667", "module": "D"}]}}, {"referenceToLCIAMethodDataSet": {"shortDescription": [{"value": "Globales Erwärmungspotenzial fossil (GWP-fossil)", "lang": "de"}, {"value": "Global Warming Potential fossil fuels (GWP-fossil)", "lang": "en"}], "type": "LCIA method data set", "refObjectId": "5f635281-343e-44fb-83df-1971b155e6b6", "uri": "../lciamethods/5f635281-343e-44fb-83df-1971b155e6b6.xml"}, "other": {"anies": [{"name": "referenceToUnitGroupDataSet", "value": {"shortDescription": [{"value": "kg CO_(2)-Äq.", "lang": "de"}], "type": "unit group data set", "refObjectId": "1ebf3012-d0db-4de2-aefd-ef30cedb0be1", "uri": "../unitgroups/1ebf3012-d0db-4de2-aefd-ef30cedb0be1.xml"}}, {"value": "25.8890029193841", "module": "A1-A3"}, {"value": "0.202098810535556", "module": "A4"}, {"value": "0.129", "module": "A5"}, {"value": "0.00324057485554099", "module": "C1"}, {"value": "0.0457388932084379", "module": "C2"}, {"value": "0.806408256227977", "module": "C3"}, {"value": "0.0123", "module": "C4"}, {"value": "-20.13130354478", "module": "D"}]}}, {"referenceToLCIAMethodDataSet": {"shortDescription": [{"value": "Globales Erwärmungspotenzial biogen (GWP-biogenic)", "lang": "de"}, {"value": "Global Warming Potential biogenic (GWP-biogenic)", "lang": "en"}], "type": "LCIA method data set", "refObjectId": "2356e1ab-0185-4db5-86e5-16de51c7485c", "uri": "../lciamethods/2356e1ab-0185-4db5-86e5-16de51c7485c.xml"}, "other": {"anies": [{"name": "referenceToUnitGroupDataSet", "value": {"shortDescription": [{"value": "kg CO_(2)-Äq.", "lang": "de"}], "type": "unit group data set", "refObjectId": "1ebf3012-d0db-4de2-aefd-ef30cedb0be1", "uri": "../unitgroups/1ebf3012-d0db-4de2-aefd-ef30cedb0be1.xml"}}, {"value": "-0.701206555210401", "module": "A1-A3"}, {"value": "0.000340049351496336", "module": "A4"}, {"value": "1.03821590055977", "module": "A5"}, {"value": "1.24914912674797E-05", "module": "C1"}, {"value": "0.000130009895261747", "module": "C2"}, {"value": "6.44653942777746E-05", "module": "C3"}, {"value": "9.76E-08", "module": "C4"}, {"value": "-0.0433303116784982", "module": "D"}]}}, {"referenceToLCIAMethodDataSet": {"shortDescription": [{"value": "Globales Erwärmungspotenzial luluc (GWP-luluc)", "lang": "de"}, {"value": "Global Warming Potential luluc (GWP-luluc)", "lang": "en"}], "type": "LCIA method data set", "refObjectId": "4331bbdb-978a-490d-8707-eeb047f01a55", "uri": "../lciamethods/4331bbdb-978a-490d-8707-eeb047f01a55.xml"}, "other": {"anies": [{"name": "referenceToUnitGroupDataSet", "value": {"shortDescription": [{"value": "kg CO_(2)-Äq.", "lang": "de"}], "type": "unit group data set", "refObjectId": "1ebf3012-d0db-4de2-aefd-ef30cedb0be1", "uri": "../unitgroups/1ebf3012-d0db-4de2-aefd-ef30cedb0be1.xml"}}, {"value": "0.00978941924855939", "module": "A1-A3"}, {"value": "0.00124827740533793", "module": "A4"}, {"value": "5.63E-05", "module": "A5"}, {"value": "1.93403893101518E-05", "module": "C1"}, {"value": "0.000276844637663634", "module": "C2"}, {"value": "1.72992394365886E-05", "module": "C3"}, {"value": "1.68E-05", "module": "C4"}, {"value": "-0.0053", "module": "D"}]}}, {"referenceToLCIAMethodDataSet": {"shortDescription": [{"value": "Abbau Potential der stratosphärischen Ozonschicht (ODP)", "lang": "de"}, {"value": "Depletion potential of the stratospheric ozone layer (ODP)", "lang": "en"}], "type": "LCIA method data set", "refObjectId": "b5c629d6-def3-11e6-bf01-fe55135034f3", "uri": "../lciamethods/b5c629d6-def3-11e6-bf01-fe55135034f3.xml"}, "other": {"anies": [{"name": "referenceToUnitGroupDataSet", "value": {"shortDescription": [{"value": "kg CFC11-Äq.", "lang": "de"}], "type": "unit group data set", "refObjectId": "d9e957c9-7309-4474-bf3a-7777df6c4e5b", "uri": "../unitgroups/d9e957c9-7309-4474-bf3a-7777df6c4e5b.xml"}}, {"value": "1.83626856556247E-09", "module": "A1-A3"}, {"value": "5.14854085701E-14", "module": "A4"}, {"value": "7.33E-13", "module": "A5"}, {"value": "7.976975641E-16", "module": "C1"}, {"value": "1.14185029863E-14", "module": "C2"}, {"value": "2.736803818771E-13", "module": "C3"}, {"value": "1.66E-12", "module": "C4"}, {"value": "-1.74242120286609E-11", "module": "D"}]}}, {"referenceToLCIAMethodDataSet": {"shortDescription": [{"value": "Versauerungspotenzial von Boden und Wasser (AP)", "lang": "de"}, {"value": "Acidification potential of land and water (AP)", "lang": "en"}], "type": "LCIA method data set", "refObjectId": "b5c611c6-def3-11e6-bf01-fe55135034f3", "uri": "../lciamethods/b5c611c6-def3-11e6-bf01-fe55135034f3.xml"}, "other": {"anies": [{"name": "referenceToUnitGroupDataSet", "value": {"shortDescription": [{"value": "mol H^(+)-Äq.", "lang": "de"}], "type": "unit group data set", "refObjectId": "42e089ac-92bf-4bf2-8ca1-5fc40d18f2ed", "uri": "../unitgroups/42e089ac-92bf-4bf2-8ca1-5fc40d18f2ed.xml"}}, {"value": "0.114888601308843", "module": "A1-A3"}, {"value": "0.000267780151460404", "module": "A4"}, {"value": "0.000947", "module": "A5"}, {"value": "1.63968616427448E-05", "module": "C1"}, {"value": "6.2169720139199E-05", "module": "C2"}, {"value": "0.000136412715963977", "module": "C3"}, {"value": "4.87E-05", "module": "C4"}, {"value": "-0.09447270726198", "module": "D"}]}}, {"referenceToLCIAMethodDataSet": {"shortDescription": [{"value": "Eutrophierungspotenzial Süßwasser (EP-freshwater)", "lang": "de"}, {"value": "Eutrophication potential aquatic freshwater (EP-freshwater)", "lang": "en"}], "type": "LCIA method data set", "refObjectId": "b53ec18f-7377-4ad3-86eb-cc3f4f276b2b", "uri": "../lciamethods/b53ec18f-7377-4ad3-86eb-cc3f4f276b2b.xml"}, "other": {"anies": [{"name": "referenceToUnitGroupDataSet", "value": {"shortDescription": [{"value": "kg P-Äq.", "lang": "de"}], "type": "unit group data set", "refObjectId": "0429039d-a61d-4590-ba67-aa4a20a810a1", "uri": "../unitgroups/0429039d-a61d-4590-ba67-aa4a20a810a1.xml"}}, {"value": "1.81096002761217E-05", "module": "A1-A3"}, {"value": "4.91883206044017E-07", "module": "A4"}, {"value": "2.2E-07", "module": "A5"}, {"value": "7.6210725751633E-09", "module": "C1"}, {"value": "1.09090517354367E-07", "module": "C2"}, {"value": "6.94367256635612E-08", "module": "C3"}, {"value": "1.3E-08", "module": "C4"}, {"value": "-9.28955867365076E-06", "module": "D"}]}}, {"referenceToLCIAMethodDataSet": {"shortDescription": [{"value": "Eutrophierungspotenzial Salzwasser (EP-marine)", "lang": "de"}, {"value": "Eutrophication potential aquatic marine (EP-marine)", "lang": "en"}], "type": "LCIA method data set", "refObjectId": "b5c619fa-def3-11e6-bf01-fe55135034f3", "uri": "../lciamethods/b5c619fa-def3-11e6-bf01-fe55135034f3.xml"}, "other": {"anies": [{"name": "referenceToUnitGroupDataSet", "value": {"shortDescription": [{"value": "kg N-Äq.", "lang": "de"}], "type": "unit group data set", "refObjectId": "d05bb823-ecdf-4686-8c40-bf1d9257859f", "uri": "../unitgroups/d05bb823-ecdf-4686-8c40-bf1d9257859f.xml"}}, {"value": "0.0175718438344532", "module": "A1-A3"}, {"value": "9.86992372826848E-05", "module": "A4"}, {"value": "0.000125", "module": "A5"}, {"value": "7.78319131910278E-06", "module": "C1"}, {"value": "2.33098206857786E-05", "module": "C2"}, {"value": "3.04481021702039E-05", "module": "C3"}, {"value": "1.23E-05", "module": "C4"}, {"value": "-0.0135673864559497", "module": "D"}]}}, {"referenceToLCIAMethodDataSet": {"shortDescription": [{"value": "Eutrophierungspotenzial Land (EP-terrestrial)", "lang": "de"}, {"value": "Eutrophication potential terrestrial (EP-terrestrial)", "lang": "en"}], "type": "LCIA method data set", "refObjectId": "b5c614d2-def3-11e6-bf01-fe55135034f3", "uri": "../lciamethods/b5c614d2-def3-11e6-bf01-fe55135034f3.xml"}, "other": {"anies": [{"name": "referenceToUnitGroupDataSet", "value": {"shortDescription": [{"value": "mol N-Äq.", "lang": "de"}], "type": "unit group data set", "refObjectId": "71b4d617-0ec9-4d3f-b65e-e438940c2401", "uri": "../unitgroups/71b4d617-0ec9-4d3f-b65e-e438940c2401.xml"}}, {"value": "0.191378265770576", "module": "A1-A3"}, {"value": "0.00117136312955702", "module": "A4"}, {"value": "1.51E-05", "module": "A5"}, {"value": "8.6156013201221E-05", "module": "C1"}, {"value": "0.000275654805965823", "module": "C2"}, {"value": "0.000634996678037325", "module": "C3"}, {"value": "0.000135", "module": "C4"}, {"value": "-0.147808089007623", "module": "D"}]}}, {"referenceToLCIAMethodDataSet": {"shortDescription": [{"value": "Bildungspotential für troposphärisches Ozon (POCP)", "lang": "de"}, {"value": "Formation potential of tropospheric ozone photochemical oxidants (POCP)", "lang": "en"}], "type": "LCIA method data set", "refObjectId": "b5c610fe-def3-11e6-bf01-fe55135034f3", "uri": "../lciamethods/b5c610fe-def3-11e6-bf01-fe55135034f3.xml"}, "other": {"anies": [{"name": "referenceToUnitGroupDataSet", "value": {"shortDescription": [{"value": "kg NMVOC-Äq.", "lang": "de"}], "type": "unit group data set", "refObjectId": "d27c25f8-fbc1-44c6-b47b-4adbae4199c6", "uri": "../unitgroups/d27c25f8-fbc1-44c6-b47b-4adbae4199c6.xml"}}, {"value": "0.0546442123458696", "module": "A1-A3"}, {"value": "0.000236512580809444", "module": "A4"}, {"value": "0.000368", "module": "A5"}, {"value": "2.17495722028385E-05", "module": "C1"}, {"value": "5.5186420159801E-05", "module": "C2"}, {"value": "8.40418628806554E-05", "module": "C3"}, {"value": "3.82E-05", "module": "C4"}, {"value": "-0.0412764557854594", "module": "D"}]}}, {"referenceToLCIAMethodDataSet": {"shortDescription": [{"value": "Potenzial für den abiotischen Abbau nicht fossiler Ressourcen (ADPE)", "lang": "de"}, {"value": "Abiotic depletion potential for non fossil resources (ADPE)", "lang": "en"}], "type": "LCIA method data set", "refObjectId": "b2ad6494-c78d-11e6-9d9d-cec0c932ce01", "uri": "../lciamethods/b2ad6494-c78d-11e6-9d9d-cec0c932ce01.xml"}, "other": {"anies": [{"name": "referenceToUnitGroupDataSet", "value": {"shortDescription": [{"value": "kg Sb-Äq.", "lang": "de"}], "type": "unit group data set", "refObjectId": "54ccd2d9-a32a-4fc2-923d-f2c8c93e89d4", "uri": "../unitgroups/54ccd2d9-a32a-4fc2-923d-f2c8c93e89d4.xml"}}, {"value": "1.79664403486502E-06", "module": "A1-A3"}, {"value": "1.51029986178518E-08", "module": "A4"}, {"value": "4.47743143262907E-06", "module": "A5"}, {"value": "2.34000769196702E-10", "module": "C1"}, {"value": "3.34956329587783E-09", "module": "C2"}, {"value": "2.14486252087923E-09", "module": "C3"}, {"value": "4.81E-10", "module": "C4"}, {"value": "-9.55230939074058E-07", "module": "D"}]}}, {"referenceToLCIAMethodDataSet": {"shortDescription": [{"value": "Potenzial für den abiotischen Abbau fossiler Brennstoffe (ADPF)", "lang": "de"}, {"value": "Abiotic depletion potential for fossil resources (ADPF)", "lang": "en"}], "type": "LCIA method data set", "refObjectId": "b2ad6110-c78d-11e6-9d9d-cec0c932ce01", "uri": "../lciamethods/b2ad6110-c78d-11e6-9d9d-cec0c932ce01.xml"}, "other": {"anies": [{"name": "referenceToUnitGroupDataSet", "value": {"shortDescription": [{"value": "MJ", "lang": "de"}], "type": "unit group data set", "refObjectId": "93a60a57-a3c8-11da-a746-0800200c9a66", "uri": "../unitgroups/93a60a57-a3c8-11da-a746-0800200c9a66.xml"}}, {"value": "351.273242775549", "module": "A1-A3"}, {"value": "2.83696905316949", "module": "A4"}, {"value": "1.65", "module": "A5"}, {"value": "0.0439550421360843", "module": "C1"}, {"value": "0.629186802732384", "module": "C2"}, {"value": "0.410222170532278", "module": "C3"}, {"value": "0.181", "module": "C4"}, {"value": "-263.083000196227", "module": "D"}]}}, {"referenceToLCIAMethodDataSet": {"shortDescription": [{"value": "Wassernutzung (WDP)", "lang": "de"}, {"value": "Water use (WDP)", "lang": "en"}], "type": "LCIA method data set", "refObjectId": "b2ad66ce-c78d-11e6-9d9d-cec0c932ce01", "uri": "../lciamethods/b2ad66ce-c78d-11e6-9d9d-cec0c932ce01.xml"}, "other": {"anies": [{"name": "referenceToUnitGroupDataSet", "value": {"shortDescription": [{"value": "m^(3) Welt-Äq. entzogen", "lang": "de"}], "type": "unit group data set", "refObjectId": "6ae2df01-888e-46c8-b17d-49fa3869b476", "uri": "../unitgroups/6ae2df01-888e-46c8-b17d-49fa3869b476.xml"}}, {"value": "3.7164579525379", "module": "A1-A3"}, {"value": "0.00109558025392889", "module": "A4"}, {"value": "0.119267252560806", "module": "A5"}, {"value": "1.69745511221227E-05", "module": "C1"}, {"value": "0.00024297925856333", "module": "C2"}, {"value": "0.0754691029277255", "module": "C3"}, {"value": "0.000102", "module": "C4"}, {"value": "-2.9917184717151", "module": "D"}]}}, {"referenceToLCIAMethodDataSet": {"shortDescription": [{"value": "Auftreten von Krankheiten aufgrund von Feinstaubemissionen (PM)", "lang": "de"}, {"value": "Incidence of disease due to PM emissions (PM)", "lang": "en"}], "type": "LCIA method data set", "refObjectId": "b5c602c6-def3-11e6-bf01-fe55135034f3", "uri": "../lciamethods/b5c602c6-def3-11e6-bf01-fe55135034f3.xml"}, "other": {"anies": [{"name": "referenceToUnitGroupDataSet", "value": {"shortDescription": [{"value": "Krankheitsfälle", "lang": "de"}], "type": "unit group data set", "refObjectId": "3883559b-648f-4afc-8ba2-0bd24f3affa3", "uri": "../unitgroups/3883559b-648f-4afc-8ba2-0bd24f3affa3.xml"}}, {"module": "A1-A3"}, {"module": "A4"}, {"module": "A5"}, {"module": "C1"}, {"module": "C2"}, {"module": "C3"}, {"module": "C4"}, {"module": "D"}]}}, {"referenceToLCIAMethodDataSet": {"shortDescription": [{"value": "Wirkung durch Exposition des Menschen mit U235 (IR)", "lang": "de"}, {"value": "Human exposure efficiency relative to U235 (IR)", "lang": "en"}], "type": "LCIA method data set", "refObjectId": "b5c632be-def3-11e6-bf01-fe55135034f3", "uri": "../lciamethods/b5c632be-def3-11e6-bf01-fe55135034f3.xml"}, "other": {"anies": [{"name": "referenceToUnitGroupDataSet", "value": {"shortDescription": [{"value": "kBq U235-Äq.", "lang": "de"}], "type": "unit group data set", "refObjectId": "456b05bf-1415-44a9-9993-02452f554c09", "uri": "../unitgroups/456b05bf-1415-44a9-9993-02452f554c09.xml"}}, {"module": "A1-A3"}, {"module": "A4"}, {"module": "A5"}, {"module": "C1"}, {"module": "C2"}, {"module": "C3"}, {"module": "C4"}, {"module": "D"}]}}, {"referenceToLCIAMethodDataSet": {"shortDescription": [{"value": "Toxizitätsvergleichseinheit für Ökosysteme (ETP-fw)", "lang": "de"}, {"value": "Comparative toxic unit for ecosystems (ETP-fw)", "lang": "en"}], "type": "LCIA method data set", "refObjectId": "ee1082d1-b0f7-43ca-a1f0-21e2a4a74511", "uri": "../lciamethods/ee1082d1-b0f7-43ca-a1f0-21e2a4a74511.xml"}, "other": {"anies": [{"name": "referenceToUnitGroupDataSet", "value": {"shortDescription": [{"value": "CTUe", "lang": "de"}], "type": "unit group data set", "refObjectId": "aa959ded-f1eb-4efb-9c5c-2d60be36b3e6", "uri": "../unitgroups/aa959ded-f1eb-4efb-9c5c-2d60be36b3e6.xml"}}, {"module": "A1-A3"}, {"module": "A4"}, {"module": "A5"}, {"module": "C1"}, {"module": "C2"}, {"module": "C3"}, {"module": "C4"}, {"module": "D"}]}}, {"referenceToLCIAMethodDataSet": {"shortDescription": [{"value": "Toxizitätsvergleichseinheit für Menschen (krebserregend) (HTP-c)", "lang": "de"}, {"value": "Comparative toxic unit for humans (carcinogenic) (HTP-c)", "lang": "en"}], "type": "LCIA method data set", "refObjectId": "2299222a-bbd8-474f-9d4f-4dd1f18aea7c", "uri": "../lciamethods/2299222a-bbd8-474f-9d4f-4dd1f18aea7c.xml"}, "other": {"anies": [{"name": "referenceToUnitGroupDataSet", "value": {"shortDescription": [{"value": "CTUh", "lang": "de"}], "type": "unit group data set", "refObjectId": "d4c9523e-2d7e-49fd-8469-998f547d3a70", "uri": "../unitgroups/d4c9523e-2d7e-49fd-8469-998f547d3a70.xml"}}, {"module": "A1-A3"}, {"module": "A4"}, {"module": "A5"}, {"module": "C1"}, {"module": "C2"}, {"module": "C3"}, {"module": "C4"}, {"module": "D"}]}}, {"referenceToLCIAMethodDataSet": {"shortDescription": [{"value": "Toxizitätsvergleichseinheit für Menschen (nicht krebserregend) (HTP-nc)", "lang": "de"}, {"value": "Comparative toxic unit for humans (noncarcinogenic) (HTP-nc)", "lang": "en"}], "type": "LCIA method data set", "refObjectId": "3af763a5-b7a1-48c9-9cee-1f223481fcef", "uri": "../lciamethods/3af763a5-b7a1-48c9-9cee-1f223481fcef.xml"}, "other": {"anies": [{"name": "referenceToUnitGroupDataSet", "value": {"shortDescription": [{"value": "CTUh", "lang": "de"}], "type": "unit group data set", "refObjectId": "d4c9523e-2d7e-49fd-8469-998f547d3a70", "uri": "../unitgroups/d4c9523e-2d7e-49fd-8469-998f547d3a70.xml"}}, {"module": "A1-A3"}, {"module": "A4"}, {"module": "A5"}, {"module": "C1"}, {"module": "C2"}, {"module": "C3"}, {"module": "C4"}, {"module": "D"}]}}, {"referenceToLCIAMethodDataSet": {"shortDescription": [{"value": "Bodenqualitätsindex (SQP)", "lang": "de"}, {"value": "Soil quality index (SQP)", "lang": "en"}], "type": "LCIA method data set", "refObjectId": "b2ad6890-c78d-11e6-9d9d-cec0c932ce01", "uri": "../lciamethods/b2ad6890-c78d-11e6-9d9d-cec0c932ce01.xml"}, "other": {"anies": [{"name": "referenceToUnitGroupDataSet", "value": {"shortDescription": [{"value": "SQP", "lang": "de"}], "type": "unit group data set", "refObjectId": "f130951c-e67f-4f7f-8dd4-665de3974e18", "uri": "../unitgroups/f130951c-e67f-4f7f-8dd4-665de3974e18.xml"}}, {"module": "A1-A3"}, {"module": "A4"}, {"module": "A5"}, {"module": "C1"}, {"module": "C2"}, {"module": "C3"}, {"module": "C4"}, {"module": "D"}]}}]}, "otherAttributes": {"{http://www.indata.network/EPD/2019}epd-version": "1.2"}, "version": "1.1", "locations": "../ILCDLocations.xml"}