{"processInformation": {"dataSetInformation": {"UUID": "d741f800-3177-4681-8095-c21f67a6d0d8", "name": {"baseName": [{"value": "Entrauchungsklappe EKM90", "lang": "de"}, {"value": "EKM90 smoke control damper", "lang": "en"}], "functionalUnitFlowProperties": [{"lang": "de"}]}, "classificationInformation": {"classification": [{"class": [{"value": "Gebäudetechnik", "level": 0, "classId": "8"}, {"value": "Klimatisierung und Lüftung", "level": 1, "classId": "8.2"}, {"value": "Zubehör", "level": 2, "classId": "8.2.03"}], "name": "OEKOBAU.DAT"}, {"class": [{"value": "03 Gebäudetechnik", "level": 0}, {"value": "Brandschutzeinrichtungen", "level": 1}, {"value": "Brandschutzklappen und Brandschutzventile und Entrauchungsklappen", "level": 2}], "name": "IBUCategories"}]}, "generalComment": [{"value": "Die wartungsfreie korrosionsbestndige Entrauchungsklappe EKM90 besteht aus einem Gehuse aus hochtemperatur-bestndigem, abriebfestem Kalziumsilikat mit einem oder mehreren innenliegenden bruchsicheren Klappenblttern. Antriebsachsen sind aus Edelstahl. Schutzgitter, als optionales Zubehr fr Entrauchungsklappen ohne Anschlussleitungen zum Schutz der Durchstrmffnungen, sind aus verzinktem Stahlblech. Der Antrieb zum Schlieen und ffnen der Entrauchungsklappe erfolgt mittels eines elektrischen Antriebsmotors. Spezielle Dichtungen ohne zustzliche Anschlge ermglichen groe freie Querschnitte, extrem geringe Druckverluste und Schallleistungspegel. Das ffnen der Entrauchungsklappe ist auch noch nach 25 Minuten Vollbrandbeanspruchung mglich.", "lang": "de"}, {"value": "The maintenance-free, corrosion-resistant EKM90 smoke control damper comprises a casing made of high temperature-resistant, abrasion-resistant calcium silicate with one or multiple internal break-proof damper blades. The drive shafts are made of stainless steel. Protective grilles, as an optional accessory for smoke control dampers without connecting ducts for protecting the flow-through openings, are made of galvanized sheet steel. The drive for closing and opening the smoke control damper is powered by an electric drive motor. Special seals without additional limit stops make for large free cross-sections, extremely low pressure drops and sound power levels. The smoke control damper can still be opened after 25 minutes of full exposure to fire.", "lang": "en"}]}, "quantitativeReference": {"referenceToReferenceFlow": [0]}, "time": {"referenceYear": 2023, "dataSetValidUntil": 2028, "other": {"anies": [{"name": "publicationDateOfEPD", "value": 1701648000000}]}}, "geography": {"locationOfOperationSupplyOrProduction": {"location": "DE"}}, "technology": {"technologyDescriptionAndIncludedProcesses": [{"value": "Die Produktion erfolgt an einem Standort im Werk Weener. Notwendige Roh- und Halbteile, Hilfs- und Betriebsstoffe werden von Lieferanten angeliefert und fließen in die Produktion mit ein. Die Fertigung der Halbteile erfolgt in einer Vorfertigung mit üblichen Fertigungsverfahren. Metallteile werden gestanzt und in Form gekantet ggf. gefräst, Teile aus Kalziumsilikat gesägt und gefräst. Zur Vermeidung von Abfällen werden Zuschnitte entsprechend optimiert. Abfälle, die dann noch entstehen, werden gesammelt und möglichst von entsprechenden Firmen recycelt oder als Hausmüll entsorgt und verbrannt. Schmierstoffe werden weitestgehend gesammelt, aufbereitet und in der Produktion wiederverwendet. Stäube und Dünste werden vor Ort abgesaugt und gesammelt. Die Teile der Vorfertigung werden zusammen mit eingekauften Teilen zu Entrauchungsklappen endmontiert, im Rahmen der Qualitätssicherung nach ISO 9001 geprüft, verpackt und ausgeliefert. \nTechnische Daten: \nDas folgende Kapitel enthlt Angaben ber die Gren und die Leistung in Stufen und Klassen in Bezug auf die entsprechenden wesentlichen Merkmale der EN 12101-8. Die vollstndige erklrte Leistung des Produktes bezglich aller wesentlichen Merkmale gem EN 12101-8 sind der Leistungserklrung der Wildeboer Bauteile GmbH zu entnehmen. Brandprfungen erfolgten nach EN 1366-10 und EN 1366-2. \nDeklarierte Einheit: \nDie Deklaration bezieht sich auf ein Stck Entrauchungsklappe EKM90 der Wildeboer Bauteile GmbH der Gre 200 mm x 200 mm x 220 mm (Gesamtgewicht 14,7 kg) inklusive kleinem elektrischen Antriebsmotor (Gewicht 0,86 kg) und Standard-Beipack (Gewicht ca. 0,3 kg).\nDie kobilanzergebnisse von Varianten oder variierenden Abmessungen des deklarierten Produkts knnen von der Wildeboer Bauteile GmbH auf Anfrage bereitgestellt werden.", "lang": "de"}, {"value": "Production is performed at a single location in the factory in Weener. The necessary raw parts and semi-finished parts as well as auxiliary and operating materials are supplied by suppliers and enter into production. The production of semi-finished parts is performed in pre-fabrication with conventional production methods. Metal parts are punched and edged into shape and, if necessary, milled . Calcium silicate parts are sawn and milled. Cuts are optimised accordingly to prevent waste. Waste which is then still produced is collected and, wherever possible, The parts from pre-fabrication are assembled in final assembly together with purchased parts to form the smoke control dampers, checked within the scope of quality assurance according to ISO 9001, packaged and dispatched. \nTechnical data: \nThe following chapter contains specifications of the sizes and performance in levels and classes in relation to the respective essential characteristics of EN 12101-8. Refer to the declaration of performance provided by Wildeboer Bauteile GmbH for the complete declared performance of the product in relation to all essential characteristics in accordance with EN 12101-8. Fire tests were performed according to EN 1366-10 and EN 1366-2. \nDeclared unit: \nThe declaration relates to a single EKM90 smoke control damper produced by Wildeboer Bauteile GmbH, size 200 mm x 200 mm x 220 mm (total weight 14.7 kg) including a small electric drive motor (weight 0.86 kg) and standard accessory kit (weight approx. 0.3 kg)\nThe eco-balance results of variants of the declared product or products with varying dimensions can be provided by Wildeboer Bauteile GmbH on request.", "lang": "en"}], "technologicalApplicability": [{"value": "Die Entrauchungsklappe EKM90 ist geeignet zum Rauchschutz, fr Entrauchungsanlagen, zur Zuluftzufhrung und in kombinierten Anlagen zur Be- und Entlftung von Gebuden. Des Weiteren ist sie anwendbar in Anlagen mit automatisch oder manuell ausgelstem ffnen oder Schlieen der Entrauchungsklappen. Nachgewiesen und zulssig sind die Betriebsstellungen \"vollstndig geffnet\", \"vollstndig geschlossen\" und beliebige Zwischenstellungen. Die Entrauchungsklappe kann verwendet werden zum Einbau in ≥95 mm dicke massive Wnde und Metallstnderwnde, in ≥90mm dicke Schachtwnde und in ≥100 mm dicke massive Decken, an und zwischen waagerecht liegenden oder senkrecht stehenden Entrauchungsleitungen. An die Entrauchungsklappe knnen Entrauchungsleitungen mit Feuerwiderstandsdauer ein- oder beidseitig angeschlossen werden; die Entrauchungsleitungen ohne Feuerwiderstandsdauer knnen nur einseitig angeschlossen werden; die Schutzgitter ein- oder beidseitig. Der Einbau erfolgt bauseits nass oder trocken. Fr weitere Informationen siehe Herstellerunterlagen.", "lang": "de"}, {"value": "The EKM90 smoke control damper is suitable for smoke protection, smoke extraction systems, air supply and in combined systems for ventilation of buildings. It is also suitable for use in systems with automatically or manually triggered opening or closing of the smoke control dampers. The operating positions \"fully opened\", \"fully closed\" and any intermediate positions have been verified and approved. The smoke control damper can be used for installation in \nrigid walls and metal stud walls with a thickness of ≥95 mm, in \nshaft walls with a thickness of ≥90 mm and in rigid ceilings with a thickness of ≥100 mm, on and between horizontal or vertical smoke extraction ducts. Smoke extraction ducts with fire resistance period can be connected to the smoke control damper on one side or both sides; the smoke extraction ducts without fire resistance period can only be connected on one side; the protective grilles on one side or both sides. Installation is performed on-site wet or dry. For further information see the manufacturers documents.", "lang": "en"}]}}, "modellingAndValidation": {"LCIMethodAndAllocation": {"typeOfDataSet": "EPD", "referenceToLCAMethodDetails": [{"shortDescription": [{"value": "Brandschutzklappen und Brandschutzventile und Entrauchungsklappen.pdf", "lang": "de"}], "type": "source data set", "refObjectId": "a7190247-4a5a-4183-a47b-dae49a692879"}], "other": {"anies": [{"name": "subType", "value": "specific dataset"}]}}, "dataSourcesTreatmentAndRepresentativeness": {"referenceToDataSource": [{"shortDescription": [{"value": "GaBi Database (all versions)", "lang": "de"}], "type": "source data set", "refObjectId": "28d74cc0-db8b-4d7e-bc44-5f6d56ce0c4a"}, {"shortDescription": [{"value": "GaBi Database Edition 2022, CUP 2022.02", "lang": "de"}], "type": "source data set", "refObjectId": "94f442cb-662e-43ea-a792-4b0a35132e93"}], "useAdviceForDataSet": [{"value": "Gültigkeitsbereich: \nDieses Dokument bezieht sich auf die Herstellung, den Transport, den Einbau, den Betrieb und die Entsorgung von Entrauchungsklappen \n(EKM90, 200x200x220mm, bestehend aus Gehuse und kleinem Antrieb) in Anlagen zur Entrauchung, zum Rauchschutz, zur Zuluftzufhrung und in kombinierten Anlagen zur Be- und Entlftung von Gebuden. Die Entrauchungsklappen werden ausschlielich in Deutschland im Werk Weener produziert, in dem die Produktionsdaten des Jahres 2022/2023 erhoben wurden. \nSystemgrenze: \nDie Systemgrenze der EPD vom Typ \"Wiege bis Bahre\" folgt dem modularen Aufbau gem EN 15804. Die kobilanz der betrachteten Produkte bercksichtigt die Module A, B, C und D:\n\nProduktstadium (A1–A3)\nRohstoffbereitstellung sowie LKW-Transport der Rohstoffe zum Werk. Produktionsaufwendungen inkl. Verpackungsmaterial. Behandlung von nicht metallischen Produktionsabfllen. Metallische Produktionsabflle erreichen das Ende der Abfalleigenschaft direkt nach dem Entstehen und werden nach Modul D exportiert.\n\nStadium der Errichtung des Bauwerks (A4–A5)\nModul A4: LKW-Transport zur Baustelle (100 km). Transportentfernung kann ggfs. auf Gebudeebene angepasst werden (z. B. bei 200 km tatschlicher Transportentfernung: Multiplikation der kobilanzwerte mit dem Faktor 2).\nModul A5: Verpackungsbehandlung. Ggfs. resultierende Gutschriften in Modul D. Stromverbrauch fr die Installation (ggfs. Einsatz von Handmaschinen) wurde nicht betrachtet.\n\nNutzungsstadium (B1–B5): \nWhrend der Nutzung des Produktes (B1) werden keine Emissionen freigesetzt. Eine Instandhaltung (B2) und Reparatur (B3) bzw. ein Austausch einzelner Komponenten (B4) ist whrend der betrachteten Nutzungsdauer nicht relevant (Wartungsfreiheit). Whrend der Nutzungsdauer ist laut Herstellerangaben keine Erneuerung des Produktes notwendig (B5). Die Module B1 bis B5 werden deshalb mit 0 deklariert.\n\nNutzungsstadium – Betrieb des Gebudes(B6–B7):\nDie fr den Betrieb des Produktes mit elektrischem Antriebsmotor erforderliche elektrische Energie sowie die elektrische Energie fr Sollwertverstellungen.\n\nEntsorgungsstadium (C1–C4)\nC1: Manueller Rckbau (lastenfrei)\nC2: LKW-Transport zur Abfallaufbereitung (50 km). Die Transportentfernung kann ggfs. auf Gebudeebene angepasst werden (z.B. bei 100 km tatschlicher Transportentfernung: Multiplikation der kobilanzwerte mit dem Faktor 2). Der End-of-waste Status der Motoren wird nach der Aufbereitung respektive Trennung der darin enthaltenen Materialfraktionen erreicht. Die Aufwnde fr die Aufbereitung wurden im Produktlebenszyklus vernachlssigt.\nModul C3: thermische Behandlung von Rohstoffen mit\nHeizwert.\nModul C4: Deponierung von Rohstoffen ohne Heizwert.\n\nGutschriften und Lasten auerhalb der Systemgrenzen (D)\nLasten und Gutschriften aus stofflichem Recycling von Metallen (inkl. Aufbereitung) und Gutschriften fr substituierte\nthermische Energie und Strom, welche aus den Modulen A1–A3, A5 und C3 exportiert wurden.", "lang": "de"}, {"value": "Scope: \nThis document refers to the manufacture, transportation, installation, operation and disposal of smoke control dampers (EKM90, 200x200x220 mm, comprising a casing and a small drive) in systems for smoke extraction, for smoke protection, for air supply and in combined systems for ventilation of buildings. The smoke control dampers are produced exclusively in Germany at the factory in Weener in which the production data from the year 2022/2023 was collected. \nSystem boundary: \nThe system boundary of the EPD of the type \"from the cradle to the grave\" follows the modular structure in accordance with EN 15804. The eco-balance of the assessed products takes into account modules A, B, C and D:\n\nProduct stage (A1–A3)\nProvision of raw materials and transportation by truck of the raw materials to the factory. Production expenses including packaging material. Treatment of non-metallic production waste. Metallic production waste reaches the end of the waste characteristic immediately after creation, and is exported according to module D.\n\nConstruction stage (A4–A5)\nModule A4: Transportation by truck to the construction site (100 km). The transportation distance can be adjusted at building level as necessary (e.g. in case of actual transportation distance of 200 km: multiplication of the eco-balance values by a factor of 2). \nModule A5: Treatment of packaging. Resultant credit notes in module D as necessary. Power consumption for installation (use of hand-held power tools as necessary) was not taken into account.\n\nUse stage (B1–B5): \nNo emissions are released during use of the product (B1). Servicing (B2) and repair (B3) or the replacement of individual components (B4) is not relevant during the assessed life span (maintenance-free). According to manufacturer information, the product does not need to be restored during the life span (B5). Modules B1 to B5 are therefore declared with a 0.\n\nUse stage – operation of the building (B6–B7):\nThe required electrical energy for operation of the product with electric drive motor and the electrical energy for set point adjustments.\n\nDisposal stage (C1–C4)\nC1: Manual demolition (unencumbered) \nC2: Transportation by truck for waste treatment (50 km). The transportation distance can be adjusted at building level as necessary (e.g. in case of actual transportation distance of 100 km: multiplication of the eco-balance values by a factor of 2). The end-of-waste status of motors is achieved after processing, or separation of the material fractions contained. The expenses for processing were neglected in the product life cycle. \nModule C3: thermal treatment of raw materials with calorific value.\nModule C4: disposal of raw materials without calorific value.\n\nCredits and debits outside the system boundaries (D)\nDebits and credits from material recycling of metals (including processing) and credits for substituted thermal energy and power which have been exported from modules A1 – A3, A5 and C3.", "lang": "en"}], "other": {"anies": [{"name": "referenceToOriginalEPD", "value": {"shortDescription": {"value": "Entrauchungsklappe EKM90.pdf", "defaultValue": "Entrauchungsklappe EKM90.pdf", "lstrings": [{"lang": "de", "value": "Entrauchungsklappe EKM90.pdf"}]}, "type": "source data set", "uuid": {"uuid": "9f6dcad9-0f76-4b70-9809-f052e19630a9"}, "refObjectId": "9f6dcad9-0f76-4b70-9809-f052e19630a9", "resourceURLs": ["https://oekobaudat.de/OEKOBAU.DAT/resource/sources/9f6dcad9-0f76-4b70-9809-f052e19630a9/Entrauchungsklappe_EKM90_20815.pdf?version=00.02.000"]}}]}}, "validation": {"review": [{"referenceToNameOfReviewerAndInstitution": [{"shortDescription": [{"value": "Institut Bauen und Umwelt e. V.", "lang": "de"}], "type": "contact data set", "refObjectId": "d111dbec-b024-4be5-86c5-752d6eb2cf95", "uri": "../contacts/d111dbec-b024-4be5-86c5-752d6eb2cf95.xml"}], "type": "Accredited third party review"}]}, "complianceDeclarations": {"compliance": [{"referenceToComplianceSystem": {"shortDescription": [{"value": "DIN EN 15804+A2", "lang": "de"}], "type": "source data set", "refObjectId": "c0016b33-8cf7-415c-ac6e-deba0d21440d", "uri": "../sources/c0016b33-8cf7-415c-ac6e-deba0d21440d.xml"}}, {"referenceToComplianceSystem": {"shortDescription": [{"value": "ISO 14025", "lang": "de"}], "type": "source data set", "refObjectId": "4f2eb655-6e44-4874-a95a-e28f5442cd4d", "uri": "../sources/4f2eb655-6e44-4874-a95a-e28f5442cd4d.xml"}}]}}, "administrativeInformation": {"commissionerAndGoal": {"referenceToCommissioner": [{"shortDescription": [{"value": "Wildeboer Bauteile GmbH", "lang": "de"}], "type": "contact data set", "refObjectId": "1412ea7e-e62c-46e9-acfa-aa7164e82837", "uri": "../contacts/1412ea7e-e62c-46e9-acfa-aa7164e82837.xml"}]}, "dataGenerator": {"referenceToPersonOrEntityGeneratingTheDataSet": [{"shortDescription": [{"value": "Sphera Solutions GmbH", "lang": "de"}], "type": "contact data set", "refObjectId": "623edf96-39d1-4e6f-9892-674c7228546b", "uri": "../contacts/623edf96-39d1-4e6f-9892-674c7228546b.xml"}]}, "dataEntryBy": {"timeStamp": 1701648000000, "referenceToDataSetFormat": [{"shortDescription": [{"value": "ILCD Format", "lang": "de"}], "type": "source data set", "refObjectId": "a97a0155-0234-4b87-b4ce-a45da52f2a40", "uri": "../sources/a97a0155-0234-4b87-b4ce-a45da52f2a40.xml"}, {"shortDescription": [{"value": "EPD-Datenformaterweiterungen v1.2", "lang": "de"}, {"value": "EPD Data Format Extensions v1.2", "lang": "en"}], "type": "source data set", "refObjectId": "a29449fd-aa2f-4de8-b5d7-4b06b43c6fde", "uri": "../sources/a29449fd-aa2f-4de8-b5d7-4b06b43c6fde.xml"}]}, "publicationAndOwnership": {"dataSetVersion": "00.08.001", "referenceToRegistrationAuthority": {"shortDescription": [{"value": "Institut Bauen und Umwelt e. V.", "lang": "de"}], "type": "contact data set", "refObjectId": "d111dbec-b024-4be5-86c5-752d6eb2cf95", "uri": "../contacts/d111dbec-b024-4be5-86c5-752d6eb2cf95.xml"}, "registrationNumber": "EPD-WIL-20230374-ICA1-DE", "referenceToOwnershipOfDataSet": {"shortDescription": [{"value": "Wildeboer Bauteile GmbH", "lang": "de"}], "type": "contact data set", "refObjectId": "1412ea7e-e62c-46e9-acfa-aa7164e82837", "uri": "../contacts/1412ea7e-e62c-46e9-acfa-aa7164e82837.xml"}, "copyright": true, "licenseType": "Free of charge for all users and uses", "accessRestrictions": [{"value": "None", "lang": "en"}], "other": {"anies": [{"name": "referenceToPublisher", "value": {"shortDescription": [{"value": "Institut Bauen und Umwelt e. V.", "lang": "de"}], "type": "contact data set", "refObjectId": "d111dbec-b024-4be5-86c5-752d6eb2cf95", "uri": "../contacts/d111dbec-b024-4be5-86c5-752d6eb2cf95.xml"}}]}}}, "exchanges": {"exchange": [{"dataSetInternalID": 0, "referenceToFlowDataSet": {"shortDescription": [{"value": "Entrauchungsklappe EKM90 (1 Stück Entrauchungsklappe EKM90 inkl. elektrischer Antriebsmotor mit 14,7 kg/Stück)", "lang": "de"}], "type": "flow data set", "refObjectId": "12b06e1f-a6ef-9bd4-444b-929a842ae32e", "uri": "../flows/12b06e1f-a6ef-9bd4-444b-929a842ae32e.xml"}, "meanAmount": 1.0, "referencesToDataSource": {}, "referenceFlow": true, "resolvedFlowVersion": "00.08.001", "resultingflowAmount": 1.0, "flowProperties": [{"name": [{"lang": "de", "value": "Anzahl"}, {"lang": "en", "value": "Number of pieces"}], "uuid": "01846770-4cfe-4a25-8ad9-919d8d378345", "referenceFlowProperty": true, "meanValue": 1.0, "referenceUnit": "pcs.", "unitGroupUUID": "934110e3-baf4-49e9-992c-3d8109a6aafb"}], "materialProperties": [{"name": "weight per piece", "value": "14.7", "unit": "kg"}], "typeOfFlow": "Product flow", "classification": {"classHierarchy": "Gebäudetechnik / Klimatisierung und Lüftung / Zubehör", "name": "OEKOBAU.DAT"}}, {"dataSetInternalID": 1, "referenceToFlowDataSet": {"shortDescription": [{"value": "Erneuerbare Primärenergie als Energieträger (PERE)", "lang": "de"}, {"value": "Renewable primary energy as energy carrier (PERE)", "lang": "en"}], "type": "flow data set", "refObjectId": "20f32be5-0398-4288-9b6d-accddd195317", "uri": "../flows/20f32be5-0398-4288-9b6d-accddd195317.xml"}, "exchange direction": "INPUT", "other": {"anies": [{"name": "referenceToUnitGroupDataSet", "value": {"shortDescription": [{"value": "MJ", "lang": "de"}], "type": "unit group data set", "refObjectId": "93a60a57-a3c8-11da-a746-0800200c9a66", "uri": "../unitgroups/93a60a57-a3c8-11da-a746-0800200c9a66.xml"}}, {"value": "53.0287219658811", "module": "A1-A3"}, {"value": "0.0691783510705806", "module": "A4"}, {"value": "26.293090543033", "module": "A5"}, {"value": "0", "module": "B1"}, {"value": "0", "module": "B2"}, {"value": "0", "module": "B3"}, {"value": "0", "module": "B4"}, {"value": "0", "module": "B5"}, {"value": "4.42806806396424", "module": "B6"}, {"value": "0", "module": "B7"}, {"value": "0", "module": "C1"}, {"value": "0.0333888584329973", "module": "C2"}, {"value": "0.0539294109037614", "module": "C3"}, {"value": "0.344744614781086", "module": "C4"}, {"value": "-9.35067950098515", "module": "D"}]}, "resolvedFlowVersion": "38.00.000", "flowProperties": [], "typeOfFlow": "Other flow", "classification": {"classHierarchy": "Quantities", "name": "GaBiCategories"}}, {"dataSetInternalID": 2, "referenceToFlowDataSet": {"shortDescription": [{"value": "Erneuerbare Primärenergie zur stofflichen Nutzung (PERM)", "lang": "de"}, {"value": "Renewable primary energy resources as material utilization (PERM)", "lang": "en"}], "type": "flow data set", "refObjectId": "fb3ec0de-548d-4508-aea5-00b73bf6f702", "uri": "../flows/fb3ec0de-548d-4508-aea5-00b73bf6f702.xml"}, "exchange direction": "INPUT", "other": {"anies": [{"name": "referenceToUnitGroupDataSet", "value": {"shortDescription": [{"value": "MJ", "lang": "de"}], "type": "unit group data set", "refObjectId": "93a60a57-a3c8-11da-a746-0800200c9a66", "uri": "../unitgroups/93a60a57-a3c8-11da-a746-0800200c9a66.xml"}}, {"value": "26.154", "module": "A1-A3"}, {"value": "0", "module": "A4"}, {"value": "-26.154", "module": "A5"}, {"value": "0", "module": "B1"}, {"value": "0", "module": "B2"}, {"value": "0", "module": "B3"}, {"value": "0", "module": "B4"}, {"value": "0", "module": "B5"}, {"value": "0", "module": "B6"}, {"value": "0", "module": "B7"}, {"value": "0", "module": "C1"}, {"value": "0", "module": "C2"}, {"value": "0", "module": "C3"}, {"value": "0", "module": "C4"}, {"value": "0", "module": "D"}]}, "resolvedFlowVersion": "38.00.000", "flowProperties": [], "typeOfFlow": "Other flow", "classification": {"classHierarchy": "Quantities", "name": "GaBiCategories"}}, {"dataSetInternalID": 3, "referenceToFlowDataSet": {"shortDescription": [{"value": "Total erneuerbare Primärenergie (PERT)", "lang": "de"}, {"value": "Total use of renewable primary energy resources (PERT)", "lang": "en"}], "type": "flow data set", "refObjectId": "53f97275-fa8a-4cdd-9024-65936002acd0", "uri": "../flows/53f97275-fa8a-4cdd-9024-65936002acd0.xml"}, "exchange direction": "INPUT", "other": {"anies": [{"name": "referenceToUnitGroupDataSet", "value": {"shortDescription": [{"value": "MJ", "lang": "de"}], "type": "unit group data set", "refObjectId": "93a60a57-a3c8-11da-a746-0800200c9a66", "uri": "../unitgroups/93a60a57-a3c8-11da-a746-0800200c9a66.xml"}}, {"value": "79.1827219658811", "module": "A1-A3"}, {"value": "0.0691783510705806", "module": "A4"}, {"value": "0.139090543033019", "module": "A5"}, {"value": "0", "module": "B1"}, {"value": "0", "module": "B2"}, {"value": "0", "module": "B3"}, {"value": "0", "module": "B4"}, {"value": "0", "module": "B5"}, {"value": "4.42806806396424", "module": "B6"}, {"value": "0", "module": "B7"}, {"value": "0", "module": "C1"}, {"value": "0.0333888584329973", "module": "C2"}, {"value": "0.0539294109037614", "module": "C3"}, {"value": "0.344744614781086", "module": "C4"}, {"value": "-9.35067950098515", "module": "D"}]}, "resolvedFlowVersion": "38.00.000", "flowProperties": [], "typeOfFlow": "Other flow", "classification": {"classHierarchy": "Quantities / Environmental quantities / EPD EN 15804 / LCI indicators", "name": "GaBiCategories"}}, {"dataSetInternalID": 4, "referenceToFlowDataSet": {"shortDescription": [{"value": "Nicht-erneuerbare Primärenergie als Energieträger (PENRE)", "lang": "de"}, {"value": "Non renewable primary energy as energy carrier (PENRE)", "lang": "en"}], "type": "flow data set", "refObjectId": "ac857178-2b45-46ec-892a-a9a4332f0372", "uri": "../flows/ac857178-2b45-46ec-892a-a9a4332f0372.xml"}, "exchange direction": "INPUT", "other": {"anies": [{"name": "referenceToUnitGroupDataSet", "value": {"shortDescription": [{"value": "MJ", "lang": "de"}], "type": "unit group data set", "refObjectId": "93a60a57-a3c8-11da-a746-0800200c9a66", "uri": "../unitgroups/93a60a57-a3c8-11da-a746-0800200c9a66.xml"}}, {"value": "247.567696326474", "module": "A1-A3"}, {"value": "1.165384427735", "module": "A4"}, {"value": "7.49971353230196", "module": "A5"}, {"value": "0", "module": "B1"}, {"value": "0", "module": "B2"}, {"value": "0", "module": "B3"}, {"value": "0", "module": "B4"}, {"value": "0", "module": "B5"}, {"value": "30.6423532841173", "module": "B6"}, {"value": "0", "module": "B7"}, {"value": "0", "module": "C1"}, {"value": "0.58873237399752", "module": "C2"}, {"value": "11.3776538307476", "module": "C3"}, {"value": "2.30071633325706", "module": "C4"}, {"value": "-76.1567360160594", "module": "D"}]}, "resolvedFlowVersion": "38.00.000", "flowProperties": [], "typeOfFlow": "Other flow", "classification": {"classHierarchy": "Quantities", "name": "GaBiCategories"}}, {"dataSetInternalID": 5, "referenceToFlowDataSet": {"shortDescription": [{"value": "Nicht-erneuerbare Primärenergie zur stofflichen Nutzung (PENRM)", "lang": "de"}, {"value": "Non renewable primary energy as material utilization (PENRM)", "lang": "en"}], "type": "flow data set", "refObjectId": "1421caa0-679d-4bf4-b282-0eb850ccae27", "uri": "../flows/1421caa0-679d-4bf4-b282-0eb850ccae27.xml"}, "exchange direction": "INPUT", "other": {"anies": [{"name": "referenceToUnitGroupDataSet", "value": {"shortDescription": [{"value": "MJ", "lang": "de"}], "type": "unit group data set", "refObjectId": "93a60a57-a3c8-11da-a746-0800200c9a66", "uri": "../unitgroups/93a60a57-a3c8-11da-a746-0800200c9a66.xml"}}, {"value": "17.9827", "module": "A1-A3"}, {"value": "0", "module": "A4"}, {"value": "-6.9", "module": "A5"}, {"value": "0", "module": "B1"}, {"value": "0", "module": "B2"}, {"value": "0", "module": "B3"}, {"value": "0", "module": "B4"}, {"value": "0", "module": "B5"}, {"value": "0", "module": "B6"}, {"value": "0", "module": "B7"}, {"value": "0", "module": "C1"}, {"value": "0", "module": "C2"}, {"value": "-11.0827", "module": "C3"}, {"value": "0", "module": "C4"}, {"value": "0", "module": "D"}]}, "resolvedFlowVersion": "38.00.000", "flowProperties": [], "typeOfFlow": "Other flow", "classification": {"classHierarchy": "Quantities", "name": "GaBiCategories"}}, {"dataSetInternalID": 6, "referenceToFlowDataSet": {"shortDescription": [{"value": "Total nicht erneuerbare Primärenergie (PENRT)", "lang": "de"}, {"value": "Total use of non renewable primary energy resources (PENRT)", "lang": "en"}], "type": "flow data set", "refObjectId": "06159210-646b-4c8d-8583-da9b3b95a6c1", "uri": "../flows/06159210-646b-4c8d-8583-da9b3b95a6c1.xml"}, "exchange direction": "INPUT", "other": {"anies": [{"name": "referenceToUnitGroupDataSet", "value": {"shortDescription": [{"value": "MJ", "lang": "de"}], "type": "unit group data set", "refObjectId": "93a60a57-a3c8-11da-a746-0800200c9a66", "uri": "../unitgroups/93a60a57-a3c8-11da-a746-0800200c9a66.xml"}}, {"value": "265.550396326466", "module": "A1-A3"}, {"value": "1.165384427735", "module": "A4"}, {"value": "0.599713532301961", "module": "A5"}, {"value": "0", "module": "B1"}, {"value": "0", "module": "B2"}, {"value": "0", "module": "B3"}, {"value": "0", "module": "B4"}, {"value": "0", "module": "B5"}, {"value": "30.6423532841175", "module": "B6"}, {"value": "0", "module": "B7"}, {"value": "0", "module": "C1"}, {"value": "0.58873237399752", "module": "C2"}, {"value": "0.294953830747589", "module": "C3"}, {"value": "2.30071633325707", "module": "C4"}, {"value": "-76.1567360160595", "module": "D"}]}, "resolvedFlowVersion": "38.00.000", "flowProperties": [], "typeOfFlow": "Other flow", "classification": {"classHierarchy": "Quantities / Environmental quantities / EPD EN 15804 / LCI indicators", "name": "GaBiCategories"}}, {"dataSetInternalID": 7, "referenceToFlowDataSet": {"shortDescription": [{"value": "Einsatz von Sekundärstoffen (SM)", "lang": "de"}, {"value": "Use of secondary material (SM)", "lang": "en"}], "type": "flow data set", "refObjectId": "c6a1f35f-2d09-4f54-8dfb-97e502e1ce92", "uri": "../flows/c6a1f35f-2d09-4f54-8dfb-97e502e1ce92.xml"}, "exchange direction": "INPUT", "other": {"anies": [{"name": "referenceToUnitGroupDataSet", "value": {"shortDescription": [{"value": "kg", "lang": "de"}], "type": "unit group data set", "refObjectId": "ad38d542-3fe9-439d-9b95-2f5f7752acaf", "uri": "../unitgroups/ad38d542-3fe9-439d-9b95-2f5f7752acaf.xml"}}, {"value": "1.28660624691901", "module": "A1-A3"}, {"value": "0", "module": "A4"}, {"value": "0", "module": "A5"}, {"value": "0", "module": "B1"}, {"value": "0", "module": "B2"}, {"value": "0", "module": "B3"}, {"value": "0", "module": "B4"}, {"value": "0", "module": "B5"}, {"value": "0", "module": "B6"}, {"value": "0", "module": "B7"}, {"value": "0", "module": "C1"}, {"value": "0", "module": "C2"}, {"value": "0", "module": "C3"}, {"value": "0", "module": "C4"}, {"value": "1.64964675308099", "module": "D"}]}, "resolvedFlowVersion": "38.00.000", "flowProperties": [], "typeOfFlow": "Other flow", "classification": {"classHierarchy": "Quantities / Environmental quantities / EPD EN 15804 / LCI indicators", "name": "GaBiCategories"}}, {"dataSetInternalID": 8, "referenceToFlowDataSet": {"shortDescription": [{"value": "Erneuerbare Sekundärbrennstoffe (RSF)", "lang": "de"}, {"value": "Use of renewable secondary fuels (RSF)", "lang": "en"}], "type": "flow data set", "refObjectId": "64333088-a55f-4aa2-9a31-c10b07816787", "uri": "../flows/64333088-a55f-4aa2-9a31-c10b07816787.xml"}, "exchange direction": "INPUT", "other": {"anies": [{"name": "referenceToUnitGroupDataSet", "value": {"shortDescription": [{"value": "MJ", "lang": "de"}], "type": "unit group data set", "refObjectId": "93a60a57-a3c8-11da-a746-0800200c9a66", "uri": "../unitgroups/93a60a57-a3c8-11da-a746-0800200c9a66.xml"}}, {"value": "0", "module": "A1-A3"}, {"value": "0", "module": "A4"}, {"value": "0", "module": "A5"}, {"value": "0", "module": "B1"}, {"value": "0", "module": "B2"}, {"value": "0", "module": "B3"}, {"value": "0", "module": "B4"}, {"value": "0", "module": "B5"}, {"value": "0", "module": "B6"}, {"value": "0", "module": "B7"}, {"value": "0", "module": "C1"}, {"value": "0", "module": "C2"}, {"value": "0", "module": "C3"}, {"value": "0", "module": "C4"}, {"value": "0", "module": "D"}]}, "resolvedFlowVersion": "38.00.000", "flowProperties": [], "typeOfFlow": "Other flow", "classification": {"classHierarchy": "Quantities / Environmental quantities / EPD EN 15804 / LCI indicators", "name": "GaBiCategories"}}, {"dataSetInternalID": 9, "referenceToFlowDataSet": {"shortDescription": [{"value": "Nicht erneuerbare Sekundärbrennstoffe (NRSF)", "lang": "de"}, {"value": "Use of non renewable secondary fuels (NRSF)", "lang": "en"}], "type": "flow data set", "refObjectId": "89def144-d39a-4287-b86f-efde453ddcb2", "uri": "../flows/89def144-d39a-4287-b86f-efde453ddcb2.xml"}, "exchange direction": "INPUT", "other": {"anies": [{"name": "referenceToUnitGroupDataSet", "value": {"shortDescription": [{"value": "MJ", "lang": "de"}], "type": "unit group data set", "refObjectId": "93a60a57-a3c8-11da-a746-0800200c9a66", "uri": "../unitgroups/93a60a57-a3c8-11da-a746-0800200c9a66.xml"}}, {"value": "0", "module": "A1-A3"}, {"value": "0", "module": "A4"}, {"value": "0", "module": "A5"}, {"value": "0", "module": "B1"}, {"value": "0", "module": "B2"}, {"value": "0", "module": "B3"}, {"value": "0", "module": "B4"}, {"value": "0", "module": "B5"}, {"value": "0", "module": "B6"}, {"value": "0", "module": "B7"}, {"value": "0", "module": "C1"}, {"value": "0", "module": "C2"}, {"value": "0", "module": "C3"}, {"value": "0", "module": "C4"}, {"value": "0", "module": "D"}]}, "resolvedFlowVersion": "38.00.000", "flowProperties": [], "typeOfFlow": "Other flow", "classification": {"classHierarchy": "Quantities / Environmental quantities / EPD EN 15804 / LCI indicators", "name": "GaBiCategories"}}, {"dataSetInternalID": 10, "referenceToFlowDataSet": {"shortDescription": [{"value": "Einsatz von Süßwasserressourcen (FW)", "lang": "de"}, {"value": "Use of net fresh water (FW)", "lang": "en"}], "type": "flow data set", "refObjectId": "3cf952c8-f3a4-461d-8c96-96456ca62246", "uri": "../flows/3cf952c8-f3a4-461d-8c96-96456ca62246.xml"}, "exchange direction": "INPUT", "other": {"anies": [{"name": "referenceToUnitGroupDataSet", "value": {"shortDescription": [{"value": "m^3", "lang": "de"}], "type": "unit group data set", "refObjectId": "cd950537-0a98-4044-9ba7-9f9a68d0a504", "uri": "../unitgroups/cd950537-0a98-4044-9ba7-9f9a68d0a504.xml"}}, {"value": "0.105015333982319", "module": "A1-A3"}, {"value": "6.03147343091631E-05", "module": "A4"}, {"value": "0.0074197270027872", "module": "A5"}, {"value": "0", "module": "B1"}, {"value": "0", "module": "B2"}, {"value": "0", "module": "B3"}, {"value": "0", "module": "B4"}, {"value": "0", "module": "B5"}, {"value": "0.00670651427673818", "module": "B6"}, {"value": "0", "module": "B7"}, {"value": "0", "module": "C1"}, {"value": "3.77610979090271E-05", "module": "C2"}, {"value": "0.00212016061350184", "module": "C3"}, {"value": "0.000583747525875755", "module": "C4"}, {"value": "-0.0414312093351983", "module": "D"}]}, "resolvedFlowVersion": "38.00.000", "flowProperties": [], "typeOfFlow": "Other flow", "classification": {"classHierarchy": "Quantities / Environmental quantities / EPD EN 15804 / LCI indicators", "name": "GaBiCategories"}}, {"dataSetInternalID": 11, "referenceToFlowDataSet": {"shortDescription": [{"value": "Gefährlicher Abfall zur Deponie (HWD)", "lang": "de"}, {"value": "Hazardous waste disposed (HWD)", "lang": "en"}], "type": "flow data set", "refObjectId": "430f9e0f-59b2-46a0-8e0d-55e0e84948fc", "uri": "../flows/430f9e0f-59b2-46a0-8e0d-55e0e84948fc.xml"}, "exchange direction": "OUTPUT", "other": {"anies": [{"name": "referenceToUnitGroupDataSet", "value": {"shortDescription": [{"value": "kg", "lang": "de"}], "type": "unit group data set", "refObjectId": "ad38d542-3fe9-439d-9b95-2f5f7752acaf", "uri": "../unitgroups/ad38d542-3fe9-439d-9b95-2f5f7752acaf.xml"}}, {"value": "1.7907346934722E-06", "module": "A1-A3"}, {"value": "5.38651496423863E-12", "module": "A4"}, {"value": "5.77469062648141E-11", "module": "A5"}, {"value": "0", "module": "B1"}, {"value": "0", "module": "B2"}, {"value": "0", "module": "B3"}, {"value": "0", "module": "B4"}, {"value": "0", "module": "B5"}, {"value": "2.19052040862775E-09", "module": "B6"}, {"value": "0", "module": "B7"}, {"value": "0", "module": "C1"}, {"value": "2.81929782690991E-12", "module": "C2"}, {"value": "3.97139676818033E-11", "module": "C3"}, {"value": "1.18137318244505E-10", "module": "C4"}, {"value": "-1.54101308966907E-09", "module": "D"}]}, "resolvedFlowVersion": "38.00.000", "flowProperties": [], "typeOfFlow": "Other flow", "classification": {"classHierarchy": "Quantities / Environmental quantities / EPD EN 15804 / LCI indicators", "name": "GaBiCategories"}}, {"dataSetInternalID": 12, "referenceToFlowDataSet": {"shortDescription": [{"value": "Entsorgter nicht gefährlicher Abfall (NHWD)", "lang": "de"}, {"value": "Non hazardous waste disposed (NHWD)", "lang": "en"}], "type": "flow data set", "refObjectId": "b29ef66b-e286-4afa-949f-62f1a7b4d7fa", "uri": "../flows/b29ef66b-e286-4afa-949f-62f1a7b4d7fa.xml"}, "exchange direction": "OUTPUT", "other": {"anies": [{"name": "referenceToUnitGroupDataSet", "value": {"shortDescription": [{"value": "kg", "lang": "de"}], "type": "unit group data set", "refObjectId": "ad38d542-3fe9-439d-9b95-2f5f7752acaf", "uri": "../unitgroups/ad38d542-3fe9-439d-9b95-2f5f7752acaf.xml"}}, {"value": "3.70177606595892", "module": "A1-A3"}, {"value": "0.000184523099014897", "module": "A4"}, {"value": "0.0207440706901086", "module": "A5"}, {"value": "0", "module": "B1"}, {"value": "0", "module": "B2"}, {"value": "0", "module": "B3"}, {"value": "0", "module": "B4"}, {"value": "0", "module": "B5"}, {"value": "0.00651091469759122", "module": "B6"}, {"value": "0", "module": "B7"}, {"value": "0", "module": "C1"}, {"value": "8.43738450696011E-05", "module": "C2"}, {"value": "0.0275481639068918", "module": "C3"}, {"value": "11.7675715752553", "module": "C4"}, {"value": "-0.342970070413279", "module": "D"}]}, "resolvedFlowVersion": "38.00.000", "flowProperties": [], "typeOfFlow": "Other flow", "classification": {"classHierarchy": "Quantities / Environmental quantities / EPD EN 15804 / LCI indicators", "name": "GaBiCategories"}}, {"dataSetInternalID": 13, "referenceToFlowDataSet": {"shortDescription": [{"value": "Entsorgter radioaktiver Abfall (RWD)", "lang": "de"}, {"value": "Radioactive waste disposed (RWD)", "lang": "en"}], "type": "flow data set", "refObjectId": "3449546e-52ad-4b39-b809-9fb77cea8ff6", "uri": "../flows/3449546e-52ad-4b39-b809-9fb77cea8ff6.xml"}, "exchange direction": "OUTPUT", "other": {"anies": [{"name": "referenceToUnitGroupDataSet", "value": {"shortDescription": [{"value": "kg", "lang": "de"}], "type": "unit group data set", "refObjectId": "ad38d542-3fe9-439d-9b95-2f5f7752acaf", "uri": "../unitgroups/ad38d542-3fe9-439d-9b95-2f5f7752acaf.xml"}}, {"value": "0.00686300833645931", "module": "A1-A3"}, {"value": "1.17203705417615E-06", "module": "A4"}, {"value": "3.5529859576517E-05", "module": "A5"}, {"value": "0", "module": "B1"}, {"value": "0", "module": "B2"}, {"value": "0", "module": "B3"}, {"value": "0", "module": "B4"}, {"value": "0", "module": "B5"}, {"value": "0.0050921900984887", "module": "B6"}, {"value": "0", "module": "B7"}, {"value": "0", "module": "C1"}, {"value": "7.25126815502637E-07", "module": "C2"}, {"value": "1.13007954784047E-05", "module": "C3"}, {"value": "2.55521364347998E-05", "module": "C4"}, {"value": "-0.00169931921241296", "module": "D"}]}, "resolvedFlowVersion": "38.00.000", "flowProperties": [], "typeOfFlow": "Other flow", "classification": {"classHierarchy": "Quantities / Environmental quantities / EPD EN 15804 / LCI indicators", "name": "GaBiCategories"}}, {"dataSetInternalID": 14, "referenceToFlowDataSet": {"shortDescription": [{"value": "Komponenten für die Wiederverwendung (CRU)", "lang": "de"}, {"value": "Components for re-use (CRU)", "lang": "en"}], "type": "flow data set", "refObjectId": "a2b32f97-3fc7-4af2-b209-525bc6426f33", "uri": "../flows/a2b32f97-3fc7-4af2-b209-525bc6426f33.xml"}, "exchange direction": "OUTPUT", "other": {"anies": [{"name": "referenceToUnitGroupDataSet", "value": {"shortDescription": [{"value": "kg", "lang": "de"}], "type": "unit group data set", "refObjectId": "ad38d542-3fe9-439d-9b95-2f5f7752acaf", "uri": "../unitgroups/ad38d542-3fe9-439d-9b95-2f5f7752acaf.xml"}}, {"value": "0", "module": "A1-A3"}, {"value": "0", "module": "A4"}, {"value": "0", "module": "A5"}, {"value": "0", "module": "B1"}, {"value": "0", "module": "B2"}, {"value": "0", "module": "B3"}, {"value": "0", "module": "B4"}, {"value": "0", "module": "B5"}, {"value": "0", "module": "B6"}, {"value": "0", "module": "B7"}, {"value": "0", "module": "C1"}, {"value": "0", "module": "C2"}, {"value": "0", "module": "C3"}, {"value": "0", "module": "C4"}, {"value": "0", "module": "D"}]}, "resolvedFlowVersion": "38.00.000", "flowProperties": [], "typeOfFlow": "Other flow", "classification": {"classHierarchy": "Quantities / Environmental quantities / EPD EN 15804 / LCI indicators", "name": "GaBiCategories"}}, {"dataSetInternalID": 15, "referenceToFlowDataSet": {"shortDescription": [{"value": "Stoffe zum Recycling (MFR)", "lang": "de"}, {"value": "Materials for recycling (MFR)", "lang": "en"}], "type": "flow data set", "refObjectId": "d7fe48a5-4103-49c8-9aae-b0b5dfdbd6ae", "uri": "../flows/d7fe48a5-4103-49c8-9aae-b0b5dfdbd6ae.xml"}, "exchange direction": "OUTPUT", "other": {"anies": [{"name": "referenceToUnitGroupDataSet", "value": {"shortDescription": [{"value": "kg", "lang": "de"}], "type": "unit group data set", "refObjectId": "ad38d542-3fe9-439d-9b95-2f5f7752acaf", "uri": "../unitgroups/ad38d542-3fe9-439d-9b95-2f5f7752acaf.xml"}}, {"value": "0.439153", "module": "A1-A3"}, {"value": "0", "module": "A4"}, {"value": "0", "module": "A5"}, {"value": "0", "module": "B1"}, {"value": "0", "module": "B2"}, {"value": "0", "module": "B3"}, {"value": "0", "module": "B4"}, {"value": "0", "module": "B5"}, {"value": "0", "module": "B6"}, {"value": "0", "module": "B7"}, {"value": "0", "module": "C1"}, {"value": "0", "module": "C2"}, {"value": "2.4971", "module": "C3"}, {"value": "0", "module": "C4"}, {"value": "0", "module": "D"}]}, "resolvedFlowVersion": "38.00.000", "flowProperties": [], "typeOfFlow": "Other flow", "classification": {"classHierarchy": "Quantities / Environmental quantities / EPD EN 15804 / LCI indicators", "name": "GaBiCategories"}}, {"dataSetInternalID": 16, "referenceToFlowDataSet": {"shortDescription": [{"value": "Stoffe für die Energierückgewinnung (MER)", "lang": "de"}, {"value": "Materials for energy recovery (MER)", "lang": "en"}], "type": "flow data set", "refObjectId": "59a9181c-3aaf-46ee-8b13-2b3723b6e447", "uri": "../flows/59a9181c-3aaf-46ee-8b13-2b3723b6e447.xml"}, "exchange direction": "OUTPUT", "other": {"anies": [{"name": "referenceToUnitGroupDataSet", "value": {"shortDescription": [{"value": "kg", "lang": "de"}], "type": "unit group data set", "refObjectId": "ad38d542-3fe9-439d-9b95-2f5f7752acaf", "uri": "../unitgroups/ad38d542-3fe9-439d-9b95-2f5f7752acaf.xml"}}, {"value": "0", "module": "A1-A3"}, {"value": "0", "module": "A4"}, {"value": "0", "module": "A5"}, {"value": "0", "module": "B1"}, {"value": "0", "module": "B2"}, {"value": "0", "module": "B3"}, {"value": "0", "module": "B4"}, {"value": "0", "module": "B5"}, {"value": "0", "module": "B6"}, {"value": "0", "module": "B7"}, {"value": "0", "module": "C1"}, {"value": "0", "module": "C2"}, {"value": "0", "module": "C3"}, {"value": "0", "module": "C4"}, {"value": "0", "module": "D"}]}, "resolvedFlowVersion": "38.00.000", "flowProperties": [], "typeOfFlow": "Other flow", "classification": {"classHierarchy": "Quantities / Environmental quantities / EPD EN 15804 / LCI indicators", "name": "GaBiCategories"}}, {"dataSetInternalID": 17, "referenceToFlowDataSet": {"shortDescription": [{"value": "Exportierte elektrische Energie (EEE)", "lang": "de"}, {"value": "Exported electrical energy (EEE)", "lang": "en"}], "type": "flow data set", "refObjectId": "4da0c987-2b76-40d6-9e9e-82a017aaaf29", "uri": "../flows/4da0c987-2b76-40d6-9e9e-82a017aaaf29.xml"}, "exchange direction": "OUTPUT", "other": {"anies": [{"name": "referenceToUnitGroupDataSet", "value": {"shortDescription": [{"value": "MJ", "lang": "de"}], "type": "unit group data set", "refObjectId": "93a60a57-a3c8-11da-a746-0800200c9a66", "uri": "../unitgroups/93a60a57-a3c8-11da-a746-0800200c9a66.xml"}}, {"value": "0", "module": "A1-A3"}, {"value": "0", "module": "A4"}, {"value": "4.80372283776443", "module": "A5"}, {"value": "0", "module": "B1"}, {"value": "0", "module": "B2"}, {"value": "0", "module": "B3"}, {"value": "0", "module": "B4"}, {"value": "0", "module": "B5"}, {"value": "0", "module": "B6"}, {"value": "0", "module": "B7"}, {"value": "0", "module": "C1"}, {"value": "0", "module": "C2"}, {"value": "1.51082215695742", "module": "C3"}, {"value": "0", "module": "C4"}, {"value": "0", "module": "D"}]}, "resolvedFlowVersion": "38.00.000", "flowProperties": [], "typeOfFlow": "Other flow", "classification": {"classHierarchy": "Quantities / Environmental quantities / EPD EN 15804 / LCI indicators", "name": "GaBiCategories"}}, {"dataSetInternalID": 18, "referenceToFlowDataSet": {"shortDescription": [{"value": "Exportierte thermische Energie (EET)", "lang": "de"}, {"value": "Exported thermal energy (EET)", "lang": "en"}], "type": "flow data set", "refObjectId": "98daf38a-7a79-46d3-9a37-2b7bd0955810", "uri": "../flows/98daf38a-7a79-46d3-9a37-2b7bd0955810.xml"}, "exchange direction": "OUTPUT", "other": {"anies": [{"name": "referenceToUnitGroupDataSet", "value": {"shortDescription": [{"value": "MJ", "lang": "de"}], "type": "unit group data set", "refObjectId": "93a60a57-a3c8-11da-a746-0800200c9a66", "uri": "../unitgroups/93a60a57-a3c8-11da-a746-0800200c9a66.xml"}}, {"value": "0", "module": "A1-A3"}, {"value": "0", "module": "A4"}, {"value": "8.60963103499673", "module": "A5"}, {"value": "0", "module": "B1"}, {"value": "0", "module": "B2"}, {"value": "0", "module": "B3"}, {"value": "0", "module": "B4"}, {"value": "0", "module": "B5"}, {"value": "0", "module": "B6"}, {"value": "0", "module": "B7"}, {"value": "0", "module": "C1"}, {"value": "0", "module": "C2"}, {"value": "2.71893495663519", "module": "C3"}, {"value": "0", "module": "C4"}, {"value": "0", "module": "D"}]}, "resolvedFlowVersion": "38.00.000", "flowProperties": [], "typeOfFlow": "Other flow", "classification": {"classHierarchy": "Quantities / Environmental quantities / EPD EN 15804 / LCI indicators", "name": "GaBiCategories"}}]}, "LCIAResults": {"LCIAResult": [{"referenceToLCIAMethodDataSet": {"shortDescription": [{"value": "Globales Erwärmungspotenzial total (GWP-total)", "lang": "de"}, {"value": "Global Warming Potential total (GWP-total)", "lang": "en"}], "type": "LCIA method data set", "refObjectId": "6a37f984-a4b3-458a-a20a-64418c145fa2", "uri": "../lciamethods/6a37f984-a4b3-458a-a20a-64418c145fa2.xml"}, "other": {"anies": [{"name": "referenceToUnitGroupDataSet", "value": {"shortDescription": [{"value": "kg CO_(2)-Äq.", "lang": "de"}], "type": "unit group data set", "refObjectId": "1ebf3012-d0db-4de2-aefd-ef30cedb0be1", "uri": "../unitgroups/1ebf3012-d0db-4de2-aefd-ef30cedb0be1.xml"}}, {"value": "17.4805997520178", "module": "A1-A3"}, {"value": "0.0880954073416908", "module": "A4"}, {"value": "3.11163141976622", "module": "A5"}, {"value": "0", "module": "B1"}, {"value": "0", "module": "B2"}, {"value": "0", "module": "B3"}, {"value": "0", "module": "B4"}, {"value": "0", "module": "B5"}, {"value": "1.44576969156204", "module": "B6"}, {"value": "0", "module": "B7"}, {"value": "0", "module": "C1"}, {"value": "0.0443178975959937", "module": "C2"}, {"value": "0.829675755597937", "module": "C3"}, {"value": "0.175739224106971", "module": "C4"}, {"value": "-6.69473131126745", "module": "D"}]}}, {"referenceToLCIAMethodDataSet": {"shortDescription": [{"value": "Globales Erwärmungspotenzial fossil (GWP-fossil)", "lang": "de"}, {"value": "Global Warming Potential fossil fuels (GWP-fossil)", "lang": "en"}], "type": "LCIA method data set", "refObjectId": "5f635281-343e-44fb-83df-1971b155e6b6", "uri": "../lciamethods/5f635281-343e-44fb-83df-1971b155e6b6.xml"}, "other": {"anies": [{"name": "referenceToUnitGroupDataSet", "value": {"shortDescription": [{"value": "kg CO_(2)-Äq.", "lang": "de"}], "type": "unit group data set", "refObjectId": "1ebf3012-d0db-4de2-aefd-ef30cedb0be1", "uri": "../unitgroups/1ebf3012-d0db-4de2-aefd-ef30cedb0be1.xml"}}, {"value": "19.9599113618204", "module": "A1-A3"}, {"value": "0.0867959176038058", "module": "A4"}, {"value": "0.507405096071316", "module": "A5"}, {"value": "0", "module": "B1"}, {"value": "0", "module": "B2"}, {"value": "0", "module": "B3"}, {"value": "0", "module": "B4"}, {"value": "0", "module": "B5"}, {"value": "1.44482306172018", "module": "B6"}, {"value": "0", "module": "B7"}, {"value": "0", "module": "C1"}, {"value": "0.0436651029172608", "module": "C2"}, {"value": "0.829603614228377", "module": "C3"}, {"value": "0.175415407581385", "module": "C4"}, {"value": "-6.70066112849973", "module": "D"}]}}, {"referenceToLCIAMethodDataSet": {"shortDescription": [{"value": "Globales Erwärmungspotenzial biogen (GWP-biogenic)", "lang": "de"}, {"value": "Global Warming Potential biogenic (GWP-biogenic)", "lang": "en"}], "type": "LCIA method data set", "refObjectId": "2356e1ab-0185-4db5-86e5-16de51c7485c", "uri": "../lciamethods/2356e1ab-0185-4db5-86e5-16de51c7485c.xml"}, "other": {"anies": [{"name": "referenceToUnitGroupDataSet", "value": {"shortDescription": [{"value": "kg CO_(2)-Äq.", "lang": "de"}], "type": "unit group data set", "refObjectId": "1ebf3012-d0db-4de2-aefd-ef30cedb0be1", "uri": "../unitgroups/1ebf3012-d0db-4de2-aefd-ef30cedb0be1.xml"}}, {"value": "-2.48713798812568", "module": "A1-A3"}, {"value": "0.000972975529990724", "module": "A4"}, {"value": "2.60422084925356", "module": "A5"}, {"value": "0", "module": "B1"}, {"value": "0", "module": "B2"}, {"value": "0", "module": "B3"}, {"value": "0", "module": "B4"}, {"value": "0", "module": "B5"}, {"value": "0.000852914869270804", "module": "B6"}, {"value": "0", "module": "B7"}, {"value": "0", "module": "C1"}, {"value": "0.00040776337110663", "module": "C2"}, {"value": "6.85825892420429E-05", "module": "C3"}, {"value": "0", "module": "C4"}, {"value": "0.00943735278684185", "module": "D"}]}}, {"referenceToLCIAMethodDataSet": {"shortDescription": [{"value": "Globales Erwärmungspotenzial luluc (GWP-luluc)", "lang": "de"}, {"value": "Global Warming Potential luluc (GWP-luluc)", "lang": "en"}], "type": "LCIA method data set", "refObjectId": "4331bbdb-978a-490d-8707-eeb047f01a55", "uri": "../lciamethods/4331bbdb-978a-490d-8707-eeb047f01a55.xml"}, "other": {"anies": [{"name": "referenceToUnitGroupDataSet", "value": {"shortDescription": [{"value": "kg CO_(2)-Äq.", "lang": "de"}], "type": "unit group data set", "refObjectId": "1ebf3012-d0db-4de2-aefd-ef30cedb0be1", "uri": "../unitgroups/1ebf3012-d0db-4de2-aefd-ef30cedb0be1.xml"}}, {"value": "0.00782637832310469", "module": "A1-A3"}, {"value": "0.00032651420789427", "module": "A4"}, {"value": "5.47444134063383E-06", "module": "A5"}, {"value": "0", "module": "B1"}, {"value": "0", "module": "B2"}, {"value": "0", "module": "B3"}, {"value": "0", "module": "B4"}, {"value": "0", "module": "B5"}, {"value": "9.37149725879081E-05", "module": "B6"}, {"value": "0", "module": "B7"}, {"value": "0", "module": "C1"}, {"value": "0.000245031307626255", "module": "C2"}, {"value": "3.55878031839736E-06", "module": "C3"}, {"value": "0.0003238165255863", "module": "C4"}, {"value": "-0.00350753555456044", "module": "D"}]}}, {"referenceToLCIAMethodDataSet": {"shortDescription": [{"value": "Abbau Potential der stratosphärischen Ozonschicht (ODP)", "lang": "de"}, {"value": "Depletion potential of the stratospheric ozone layer (ODP)", "lang": "en"}], "type": "LCIA method data set", "refObjectId": "b5c629d6-def3-11e6-bf01-fe55135034f3", "uri": "../lciamethods/b5c629d6-def3-11e6-bf01-fe55135034f3.xml"}, "other": {"anies": [{"name": "referenceToUnitGroupDataSet", "value": {"shortDescription": [{"value": "kg CFC11-Äq.", "lang": "de"}], "type": "unit group data set", "refObjectId": "d9e957c9-7309-4474-bf3a-7777df6c4e5b", "uri": "../unitgroups/d9e957c9-7309-4474-bf3a-7777df6c4e5b.xml"}}, {"value": "3.04668377780232E-10", "module": "A1-A3"}, {"value": "1.24957269813972E-14", "module": "A4"}, {"value": "2.17389223586231E-13", "module": "A5"}, {"value": "0", "module": "B1"}, {"value": "0", "module": "B2"}, {"value": "0", "module": "B3"}, {"value": "0", "module": "B4"}, {"value": "0", "module": "B5"}, {"value": "1.42716199524396E-11", "module": "B6"}, {"value": "0", "module": "B7"}, {"value": "0", "module": "C1"}, {"value": "2.63312192144579E-15", "module": "C2"}, {"value": "9.31314838640776E-14", "module": "C3"}, {"value": "4.1211314286368E-13", "module": "C4"}, {"value": "-6.95831285289533E-12", "module": "D"}]}}, {"referenceToLCIAMethodDataSet": {"shortDescription": [{"value": "Versauerungspotenzial von Boden und Wasser (AP)", "lang": "de"}, {"value": "Acidification potential of land and water (AP)", "lang": "en"}], "type": "LCIA method data set", "refObjectId": "b5c611c6-def3-11e6-bf01-fe55135034f3", "uri": "../lciamethods/b5c611c6-def3-11e6-bf01-fe55135034f3.xml"}, "other": {"anies": [{"name": "referenceToUnitGroupDataSet", "value": {"shortDescription": [{"value": "mol H^(+)-Äq.", "lang": "de"}], "type": "unit group data set", "refObjectId": "42e089ac-92bf-4bf2-8ca1-5fc40d18f2ed", "uri": "../unitgroups/42e089ac-92bf-4bf2-8ca1-5fc40d18f2ed.xml"}}, {"value": "0.0935123160343464", "module": "A1-A3"}, {"value": "7.54805746050885E-05", "module": "A4"}, {"value": "0.000418413460751898", "module": "A5"}, {"value": "0", "module": "B1"}, {"value": "0", "module": "B2"}, {"value": "0", "module": "B3"}, {"value": "0", "module": "B4"}, {"value": "0", "module": "B5"}, {"value": "0.00212195698503038", "module": "B6"}, {"value": "0", "module": "B7"}, {"value": "0", "module": "C1"}, {"value": "4.18273754059897E-05", "module": "C2"}, {"value": "0.000639977196380049", "module": "C3"}, {"value": "0.00124374253956918", "module": "C4"}, {"value": "-0.0295461661952515", "module": "D"}]}}, {"referenceToLCIAMethodDataSet": {"shortDescription": [{"value": "Eutrophierungspotenzial Süßwasser (EP-freshwater)", "lang": "de"}, {"value": "Eutrophication potential aquatic freshwater (EP-freshwater)", "lang": "en"}], "type": "LCIA method data set", "refObjectId": "b53ec18f-7377-4ad3-86eb-cc3f4f276b2b", "uri": "../lciamethods/b53ec18f-7377-4ad3-86eb-cc3f4f276b2b.xml"}, "other": {"anies": [{"name": "referenceToUnitGroupDataSet", "value": {"shortDescription": [{"value": "kg P-Äq.", "lang": "de"}], "type": "unit group data set", "refObjectId": "0429039d-a61d-4590-ba67-aa4a20a810a1", "uri": "../unitgroups/0429039d-a61d-4590-ba67-aa4a20a810a1.xml"}}, {"value": "4.99240807737998E-05", "module": "A1-A3"}, {"value": "1.81002563561796E-07", "module": "A4"}, {"value": "5.17822098533761E-08", "module": "A5"}, {"value": "0", "module": "B1"}, {"value": "0", "module": "B2"}, {"value": "0", "module": "B3"}, {"value": "0", "module": "B4"}, {"value": "0", "module": "B5"}, {"value": "6.48362213029158E-07", "module": "B6"}, {"value": "0", "module": "B7"}, {"value": "0", "module": "C1"}, {"value": "1.31188382550858E-07", "module": "C2"}, {"value": "2.80284785097084E-08", "module": "C3"}, {"value": "2.97319646749624E-07", "module": "C4"}, {"value": "-4.19595256934378E-06", "module": "D"}]}}, {"referenceToLCIAMethodDataSet": {"shortDescription": [{"value": "Eutrophierungspotenzial Salzwasser (EP-marine)", "lang": "de"}, {"value": "Eutrophication potential aquatic marine (EP-marine)", "lang": "en"}], "type": "LCIA method data set", "refObjectId": "b5c619fa-def3-11e6-bf01-fe55135034f3", "uri": "../lciamethods/b5c619fa-def3-11e6-bf01-fe55135034f3.xml"}, "other": {"anies": [{"name": "referenceToUnitGroupDataSet", "value": {"shortDescription": [{"value": "kg N-Äq.", "lang": "de"}], "type": "unit group data set", "refObjectId": "d05bb823-ecdf-4686-8c40-bf1d9257859f", "uri": "../unitgroups/d05bb823-ecdf-4686-8c40-bf1d9257859f.xml"}}, {"value": "0.0135043799852398", "module": "A1-A3"}, {"value": "2.39996105393468E-05", "module": "A4"}, {"value": "0.000131421086711558", "module": "A5"}, {"value": "0", "module": "B1"}, {"value": "0", "module": "B2"}, {"value": "0", "module": "B3"}, {"value": "0", "module": "B4"}, {"value": "0", "module": "B5"}, {"value": "0.000579953055794698", "module": "B6"}, {"value": "0", "module": "B7"}, {"value": "0", "module": "C1"}, {"value": "1.30315948087886E-05", "module": "C2"}, {"value": "0.00031630557246774", "module": "C3"}, {"value": "0.00031801729772195", "module": "C4"}, {"value": "-0.00390531684424854", "module": "D"}]}}, {"referenceToLCIAMethodDataSet": {"shortDescription": [{"value": "Eutrophierungspotenzial Land (EP-terrestrial)", "lang": "de"}, {"value": "Eutrophication potential terrestrial (EP-terrestrial)", "lang": "en"}], "type": "LCIA method data set", "refObjectId": "b5c614d2-def3-11e6-bf01-fe55135034f3", "uri": "../lciamethods/b5c614d2-def3-11e6-bf01-fe55135034f3.xml"}, "other": {"anies": [{"name": "referenceToUnitGroupDataSet", "value": {"shortDescription": [{"value": "mol N-Äq.", "lang": "de"}], "type": "unit group data set", "refObjectId": "71b4d617-0ec9-4d3f-b65e-e438940c2401", "uri": "../unitgroups/71b4d617-0ec9-4d3f-b65e-e438940c2401.xml"}}, {"value": "0.144531745395757", "module": "A1-A3"}, {"value": "0.000289636727071127", "module": "A4"}, {"value": "0.00198847506648445", "module": "A5"}, {"value": "0", "module": "B1"}, {"value": "0", "module": "B2"}, {"value": "0", "module": "B3"}, {"value": "0", "module": "B4"}, {"value": "0", "module": "B5"}, {"value": "0.00619785441649057", "module": "B6"}, {"value": "0", "module": "B7"}, {"value": "0", "module": "C1"}, {"value": "0.000156537865809302", "module": "C2"}, {"value": "0.00358315249247165", "module": "C3"}, {"value": "0.00349442877687556", "module": "C4"}, {"value": "-0.0425937877303807", "module": "D"}]}}, {"referenceToLCIAMethodDataSet": {"shortDescription": [{"value": "Bildungspotential für troposphärisches Ozon (POCP)", "lang": "de"}, {"value": "Formation potential of tropospheric ozone photochemical oxidants (POCP)", "lang": "en"}], "type": "LCIA method data set", "refObjectId": "b5c610fe-def3-11e6-bf01-fe55135034f3", "uri": "../lciamethods/b5c610fe-def3-11e6-bf01-fe55135034f3.xml"}, "other": {"anies": [{"name": "referenceToUnitGroupDataSet", "value": {"shortDescription": [{"value": "kg NMVOC-Äq.", "lang": "de"}], "type": "unit group data set", "refObjectId": "d27c25f8-fbc1-44c6-b47b-4adbae4199c6", "uri": "../unitgroups/d27c25f8-fbc1-44c6-b47b-4adbae4199c6.xml"}}, {"value": "0.0419100856442427", "module": "A1-A3"}, {"value": "6.52303105350997E-05", "module": "A4"}, {"value": "0.000359300747118623", "module": "A5"}, {"value": "0", "module": "B1"}, {"value": "0", "module": "B2"}, {"value": "0", "module": "B3"}, {"value": "0", "module": "B4"}, {"value": "0", "module": "B5"}, {"value": "0.00163801745859711", "module": "B6"}, {"value": "0", "module": "B7"}, {"value": "0", "module": "C1"}, {"value": "3.64454095659001E-05", "module": "C2"}, {"value": "0.000810722197690289", "module": "C3"}, {"value": "0.00096646516857288", "module": "C4"}, {"value": "-0.0125508046536814", "module": "D"}]}}, {"referenceToLCIAMethodDataSet": {"shortDescription": [{"value": "Potenzial für den abiotischen Abbau nicht fossiler Ressourcen (ADPE)", "lang": "de"}, {"value": "Abiotic depletion potential for non fossil resources (ADPE)", "lang": "en"}], "type": "LCIA method data set", "refObjectId": "b2ad6494-c78d-11e6-9d9d-cec0c932ce01", "uri": "../lciamethods/b2ad6494-c78d-11e6-9d9d-cec0c932ce01.xml"}, "other": {"anies": [{"name": "referenceToUnitGroupDataSet", "value": {"shortDescription": [{"value": "kg Sb-Äq.", "lang": "de"}], "type": "unit group data set", "refObjectId": "54ccd2d9-a32a-4fc2-923d-f2c8c93e89d4", "uri": "../unitgroups/54ccd2d9-a32a-4fc2-923d-f2c8c93e89d4.xml"}}, {"value": "0.00118687798653487", "module": "A1-A3"}, {"value": "9.04765636402996E-09", "module": "A4"}, {"value": "5.297722432033E-09", "module": "A5"}, {"value": "0", "module": "B1"}, {"value": "0", "module": "B2"}, {"value": "0", "module": "B3"}, {"value": "0", "module": "B4"}, {"value": "0", "module": "B5"}, {"value": "1.71843156103549E-07", "module": "B6"}, {"value": "0", "module": "B7"}, {"value": "0", "module": "C1"}, {"value": "3.67408480531059E-09", "module": "C2"}, {"value": "2.46112712109675E-09", "module": "C3"}, {"value": "1.79765247530643E-08", "module": "C4"}, {"value": "-0.000246818341119685", "module": "D"}]}}, {"referenceToLCIAMethodDataSet": {"shortDescription": [{"value": "Potenzial für den abiotischen Abbau fossiler Brennstoffe (ADPF)", "lang": "de"}, {"value": "Abiotic depletion potential for fossil resources (ADPF)", "lang": "en"}], "type": "LCIA method data set", "refObjectId": "b2ad6110-c78d-11e6-9d9d-cec0c932ce01", "uri": "../lciamethods/b2ad6110-c78d-11e6-9d9d-cec0c932ce01.xml"}, "other": {"anies": [{"name": "referenceToUnitGroupDataSet", "value": {"shortDescription": [{"value": "MJ", "lang": "de"}], "type": "unit group data set", "refObjectId": "93a60a57-a3c8-11da-a746-0800200c9a66", "uri": "../unitgroups/93a60a57-a3c8-11da-a746-0800200c9a66.xml"}}, {"value": "264.619017341826", "module": "A1-A3"}, {"value": "1.16417071703422", "module": "A4"}, {"value": "0.59924091709707", "module": "A5"}, {"value": "0", "module": "B1"}, {"value": "0", "module": "B2"}, {"value": "0", "module": "B3"}, {"value": "0", "module": "B4"}, {"value": "0", "module": "B5"}, {"value": "30.6363914998715", "module": "B6"}, {"value": "0", "module": "B7"}, {"value": "0", "module": "C1"}, {"value": "0.58732767358556", "module": "C2"}, {"value": "0.29485016165919", "module": "C3"}, {"value": "2.29791810512151", "module": "C4"}, {"value": "-75.9032205194232", "module": "D"}]}}, {"referenceToLCIAMethodDataSet": {"shortDescription": [{"value": "Wassernutzung (WDP)", "lang": "de"}, {"value": "Water use (WDP)", "lang": "en"}], "type": "LCIA method data set", "refObjectId": "b2ad66ce-c78d-11e6-9d9d-cec0c932ce01", "uri": "../lciamethods/b2ad66ce-c78d-11e6-9d9d-cec0c932ce01.xml"}, "other": {"anies": [{"name": "referenceToUnitGroupDataSet", "value": {"shortDescription": [{"value": "m^(3) Welt-Äq. entzogen", "lang": "de"}], "type": "unit group data set", "refObjectId": "6ae2df01-888e-46c8-b17d-49fa3869b476", "uri": "../unitgroups/6ae2df01-888e-46c8-b17d-49fa3869b476.xml"}}, {"value": "3.88413486320096", "module": "A1-A3"}, {"value": "0.000345163998500406", "module": "A4"}, {"value": "0.315863112179375", "module": "A5"}, {"value": "0", "module": "B1"}, {"value": "0", "module": "B2"}, {"value": "0", "module": "B3"}, {"value": "0", "module": "B4"}, {"value": "0", "module": "B5"}, {"value": "0.10788633755891", "module": "B6"}, {"value": "0", "module": "B7"}, {"value": "0", "module": "C1"}, {"value": "0.000394224303894335", "module": "C2"}, {"value": "0.0899572330585346", "module": "C3"}, {"value": "0.0192336884900394", "module": "C4"}, {"value": "-1.22404151988471", "module": "D"}]}}, {"referenceToLCIAMethodDataSet": {"shortDescription": [{"value": "Auftreten von Krankheiten aufgrund von Feinstaubemissionen (PM)", "lang": "de"}, {"value": "Incidence of disease due to PM emissions (PM)", "lang": "en"}], "type": "LCIA method data set", "refObjectId": "b5c602c6-def3-11e6-bf01-fe55135034f3", "uri": "../lciamethods/b5c602c6-def3-11e6-bf01-fe55135034f3.xml"}, "other": {"anies": [{"name": "referenceToUnitGroupDataSet", "value": {"shortDescription": [{"value": "Krankheitsfälle", "lang": "de"}], "type": "unit group data set", "refObjectId": "3883559b-648f-4afc-8ba2-0bd24f3affa3", "uri": "../unitgroups/3883559b-648f-4afc-8ba2-0bd24f3affa3.xml"}}, {"value": "1.33557672187997E-06", "module": "A1-A3"}, {"value": "4.70175123144985E-10", "module": "A4"}, {"value": "2.10082583879945E-09", "module": "A5"}, {"value": "0", "module": "B1"}, {"value": "0", "module": "B2"}, {"value": "0", "module": "B3"}, {"value": "0", "module": "B4"}, {"value": "0", "module": "B5"}, {"value": "1.89579460861118E-08", "module": "B6"}, {"value": "0", "module": "B7"}, {"value": "0", "module": "C1"}, {"value": "2.53016051305953E-10", "module": "C2"}, {"value": "2.12147000593977E-09", "module": "C3"}, {"value": "1.53056810543694E-08", "module": "C4"}, {"value": "-4.05281528948321E-07", "module": "D"}]}}, {"referenceToLCIAMethodDataSet": {"shortDescription": [{"value": "Wirkung durch Exposition des Menschen mit U235 (IR)", "lang": "de"}, {"value": "Human exposure efficiency relative to U235 (IR)", "lang": "en"}], "type": "LCIA method data set", "refObjectId": "b5c632be-def3-11e6-bf01-fe55135034f3", "uri": "../lciamethods/b5c632be-def3-11e6-bf01-fe55135034f3.xml"}, "other": {"anies": [{"name": "referenceToUnitGroupDataSet", "value": {"shortDescription": [{"value": "kBq U235-Äq.", "lang": "de"}], "type": "unit group data set", "refObjectId": "456b05bf-1415-44a9-9993-02452f554c09", "uri": "../unitgroups/456b05bf-1415-44a9-9993-02452f554c09.xml"}}, {"value": "0.775339418555183", "module": "A1-A3"}, {"value": "0.000113967436334104", "module": "A4"}, {"value": "0.00582370056288981", "module": "A5"}, {"value": "0", "module": "B1"}, {"value": "0", "module": "B2"}, {"value": "0", "module": "B3"}, {"value": "0", "module": "B4"}, {"value": "0", "module": "B5"}, {"value": "0.745397009572614", "module": "B6"}, {"value": "0", "module": "B7"}, {"value": "0", "module": "C1"}, {"value": "0.000106260783427821", "module": "C2"}, {"value": "0.00173785136148447", "module": "C3"}, {"value": "0.00283649868187048", "module": "C4"}, {"value": "-0.306445869503394", "module": "D"}]}}, {"referenceToLCIAMethodDataSet": {"shortDescription": [{"value": "Toxizitätsvergleichseinheit für Ökosysteme (ETP-fw)", "lang": "de"}, {"value": "Comparative toxic unit for ecosystems (ETP-fw)", "lang": "en"}], "type": "LCIA method data set", "refObjectId": "ee1082d1-b0f7-43ca-a1f0-21e2a4a74511", "uri": "../lciamethods/ee1082d1-b0f7-43ca-a1f0-21e2a4a74511.xml"}, "other": {"anies": [{"name": "referenceToUnitGroupDataSet", "value": {"shortDescription": [{"value": "CTUe", "lang": "de"}], "type": "unit group data set", "refObjectId": "aa959ded-f1eb-4efb-9c5c-2d60be36b3e6", "uri": "../unitgroups/aa959ded-f1eb-4efb-9c5c-2d60be36b3e6.xml"}}, {"value": "106.267493094743", "module": "A1-A3"}, {"value": "0.922808993719328", "module": "A4"}, {"value": "0.265683632164107", "module": "A5"}, {"value": "0", "module": "B1"}, {"value": "0", "module": "B2"}, {"value": "0", "module": "B3"}, {"value": "0", "module": "B4"}, {"value": "0", "module": "B5"}, {"value": "9.38283436512464", "module": "B6"}, {"value": "0", "module": "B7"}, {"value": "0", "module": "C1"}, {"value": "0.407750771744387", "module": "C2"}, {"value": "0.126753544121388", "module": "C3"}, {"value": "1.28731149647137", "module": "C4"}, {"value": "-30.7429225600676", "module": "D"}]}}, {"referenceToLCIAMethodDataSet": {"shortDescription": [{"value": "Toxizitätsvergleichseinheit für Menschen (krebserregend) (HTP-c)", "lang": "de"}, {"value": "Comparative toxic unit for humans (carcinogenic) (HTP-c)", "lang": "en"}], "type": "LCIA method data set", "refObjectId": "2299222a-bbd8-474f-9d4f-4dd1f18aea7c", "uri": "../lciamethods/2299222a-bbd8-474f-9d4f-4dd1f18aea7c.xml"}, "other": {"anies": [{"name": "referenceToUnitGroupDataSet", "value": {"shortDescription": [{"value": "CTUh", "lang": "de"}], "type": "unit group data set", "refObjectId": "d4c9523e-2d7e-49fd-8469-998f547d3a70", "uri": "../unitgroups/d4c9523e-2d7e-49fd-8469-998f547d3a70.xml"}}, {"value": "1.6984963187099E-06", "module": "A1-A3"}, {"value": "1.83258040353775E-11", "module": "A4"}, {"value": "1.93627682058598E-11", "module": "A5"}, {"value": "0", "module": "B1"}, {"value": "0", "module": "B2"}, {"value": "0", "module": "B3"}, {"value": "0", "module": "B4"}, {"value": "0", "module": "B5"}, {"value": "1.72705634121353E-10", "module": "B6"}, {"value": "0", "module": "B7"}, {"value": "0", "module": "C1"}, {"value": "8.21828541685609E-12", "module": "C2"}, {"value": "8.0006813702762E-12", "module": "C3"}, {"value": "1.96485748153029E-10", "module": "C4"}, {"value": "-9.08279743904628E-09", "module": "D"}]}}, {"referenceToLCIAMethodDataSet": {"shortDescription": [{"value": "Toxizitätsvergleichseinheit für Menschen (nicht krebserregend) (HTP-nc)", "lang": "de"}, {"value": "Comparative toxic unit for humans (noncarcinogenic) (HTP-nc)", "lang": "en"}], "type": "LCIA method data set", "refObjectId": "3af763a5-b7a1-48c9-9cee-1f223481fcef", "uri": "../lciamethods/3af763a5-b7a1-48c9-9cee-1f223481fcef.xml"}, "other": {"anies": [{"name": "referenceToUnitGroupDataSet", "value": {"shortDescription": [{"value": "CTUh", "lang": "de"}], "type": "unit group data set", "refObjectId": "d4c9523e-2d7e-49fd-8469-998f547d3a70", "uri": "../unitgroups/d4c9523e-2d7e-49fd-8469-998f547d3a70.xml"}}, {"value": "6.0750755430206E-07", "module": "A1-A3"}, {"value": "9.10214895475178E-10", "module": "A4"}, {"value": "6.65007649164186E-10", "module": "A5"}, {"value": "0", "module": "B1"}, {"value": "0", "module": "B2"}, {"value": "0", "module": "B3"}, {"value": "0", "module": "B4"}, {"value": "0", "module": "B5"}, {"value": "8.78590076281856E-09", "module": "B6"}, {"value": "0", "module": "B7"}, {"value": "0", "module": "C1"}, {"value": "4.25188207806453E-10", "module": "C2"}, {"value": "4.9769093288162E-10", "module": "C3"}, {"value": "2.1758860324822E-08", "module": "C4"}, {"value": "-5.18890214496139E-08", "module": "D"}]}}, {"referenceToLCIAMethodDataSet": {"shortDescription": [{"value": "Bodenqualitätsindex (SQP)", "lang": "de"}, {"value": "Soil quality index (SQP)", "lang": "en"}], "type": "LCIA method data set", "refObjectId": "b2ad6890-c78d-11e6-9d9d-cec0c932ce01", "uri": "../lciamethods/b2ad6890-c78d-11e6-9d9d-cec0c932ce01.xml"}, "other": {"anies": [{"name": "referenceToUnitGroupDataSet", "value": {"shortDescription": [{"value": "SQP", "lang": "de"}], "type": "unit group data set", "refObjectId": "f130951c-e67f-4f7f-8dd4-665de3974e18", "uri": "../unitgroups/f130951c-e67f-4f7f-8dd4-665de3974e18.xml"}}, {"value": "300.785882913659", "module": "A1-A3"}, {"value": "0.36568567783612", "module": "A4"}, {"value": "0.177873566807863", "module": "A5"}, {"value": "0", "module": "B1"}, {"value": "0", "module": "B2"}, {"value": "0", "module": "B3"}, {"value": "0", "module": "B4"}, {"value": "0", "module": "B5"}, {"value": "2.81229636291024", "module": "B6"}, {"value": "0", "module": "B7"}, {"value": "0", "module": "C1"}, {"value": "0.202098500954011", "module": "C2"}, {"value": "0.0604965197925448", "module": "C3"}, {"value": "0.477996470187916", "module": "C4"}, {"value": "-8.86644522726222", "module": "D"}]}}]}, "otherAttributes": {"{http://www.indata.network/EPD/2019}epd-version": "1.2"}, "version": "1.1", "locations": "../ILCDLocations.xml"}