{"processInformation": {"dataSetInformation": {"UUID": "e90e8a9f-5ab6-4b45-bd21-f059c0d81c72", "name": {"baseName": [{"value": "Secutex® Green G1 (biodegradable, mechanically bonded nonwoven, Naue GmbH & Co. KG)", "lang": "en"}, {"value": "Secutex® Green G1 (Biologisch abbaubares, mechanisch verfestigtes Vlies, Naue GmbH & Co. KG)", "lang": "de"}]}, "classificationInformation": {"classification": [{"class": [{"value": "Kunststoffe", "level": 0, "classId": "6"}, {"value": "Folien und Vliese", "level": 1, "classId": "6.6"}, {"value": "Technische Textilien", "level": 2, "classId": "6.6.07"}], "name": "OEKOBAU.DAT"}, {"class": [{"value": "civil engineering, earthworks, waste disposal", "level": 0, "classId": "10000000"}, {"value": "drainage fleece, soil reinforcement", "level": 1, "classId": "10200000"}, {"value": "fleece", "level": 2, "classId": "10200500"}, {"value": "non-woven geotextile", "level": 3, "classId": "10200525"}], "name": "freeclass"}]}, "generalComment": [{"value": "This EPD (type: Cradle-to-gate with modules C1-C4 and module D (A1-A3, C, D)) is based on the life cycle assessment of the Secutex® Green G1 Geotextile produced by Naue GmbH & Co. KG. This EPD is for 5 different variations of the product, based on a scaling method. Kiwa-Ecobility Experts assumes no liability for manufacturer's information, LCA data and evidence.\r\nNote: The flow and material properties as well as the environmental impact indicator results shown in this dataset refer specifically to the product Secutex® Green 60G1 (GRK4). Results for other products covered by the EPD can be found in the full EPD document.", "lang": "en"}], "other": {"anies": [{}, {"scenario": [{"description": [{"value": "Since the raw material is supplied by one supplier, the distances for transport could be accurately determined. However, since no specific transport information is available, for all truck transports (suppliers, disposal transports and internal transports) a payload factor of 50%, is used for large HGVs (loading capacity ‘>32t’), which effectively corresponds to delivering full and going back empty. The return journey and the payload factor have already been incorporated into the Ecoinvent transport processes. The supplier of the raw material has provided a confidential Life Cycle Assessment report for the purpose of conducting an EPD for Secutex® Green V01 that includes the necessary data on environmental impact categories. The results of that report, created by Quantis, are grouped into three principal categories, which are the raw materials, the production of the fiber, and the waste generated during the production process. All three of these categories have also been considered in this LCA. The electricity mix was chosen according to the geographical reference area (Germany) and time reference. As only the conventional electricity mix is used, no other energy sources were considered. No CO2 certificates were taken into account. The product can be left in the soil, which is why no inputs are necessary or have been considered for Module C1.", "lang": "en"}], "name": "Standard scenario", "default": true}]}, "<ns11:modules xmlns:ns11=\"http://openlca.org/epd_ilcd\" xmlns=\"http://lca.jrc.it/ILCD/Process\" xmlns:c=\"http://lca.jrc.it/ILCD/Contact\" xmlns:common=\"http://lca.jrc.it/ILCD/Common\" xmlns:epd=\"http://www.iai.kit.edu/EPD/2013\" xmlns:epd2=\"http://www.indata.network/EPD/2019\" xmlns:f=\"http://lca.jrc.it/ILCD/Flow\" xmlns:fp=\"http://lca.jrc.it/ILCD/FlowProperty\" xmlns:m=\"http://lca.jrc.it/ILCD/LCIAMethod\" xmlns:s=\"http://lca.jrc.it/ILCD/Source\" xmlns:u=\"http://lca.jrc.it/ILCD/UnitGroup\" name=\"A1\" scenario=\"Standard scenario\"/>", "<ns11:modules xmlns:ns11=\"http://openlca.org/epd_ilcd\" xmlns=\"http://lca.jrc.it/ILCD/Process\" xmlns:c=\"http://lca.jrc.it/ILCD/Contact\" xmlns:common=\"http://lca.jrc.it/ILCD/Common\" xmlns:epd=\"http://www.iai.kit.edu/EPD/2013\" xmlns:epd2=\"http://www.indata.network/EPD/2019\" xmlns:f=\"http://lca.jrc.it/ILCD/Flow\" xmlns:fp=\"http://lca.jrc.it/ILCD/FlowProperty\" xmlns:m=\"http://lca.jrc.it/ILCD/LCIAMethod\" xmlns:s=\"http://lca.jrc.it/ILCD/Source\" xmlns:u=\"http://lca.jrc.it/ILCD/UnitGroup\" name=\"A2\" scenario=\"Standard scenario\"/>", "<ns11:modules xmlns:ns11=\"http://openlca.org/epd_ilcd\" xmlns=\"http://lca.jrc.it/ILCD/Process\" xmlns:c=\"http://lca.jrc.it/ILCD/Contact\" xmlns:common=\"http://lca.jrc.it/ILCD/Common\" xmlns:epd=\"http://www.iai.kit.edu/EPD/2013\" xmlns:epd2=\"http://www.indata.network/EPD/2019\" xmlns:f=\"http://lca.jrc.it/ILCD/Flow\" xmlns:fp=\"http://lca.jrc.it/ILCD/FlowProperty\" xmlns:m=\"http://lca.jrc.it/ILCD/LCIAMethod\" xmlns:s=\"http://lca.jrc.it/ILCD/Source\" xmlns:u=\"http://lca.jrc.it/ILCD/UnitGroup\" name=\"A3\" scenario=\"Standard scenario\"/>", "<ns11:modules xmlns:ns11=\"http://openlca.org/epd_ilcd\" xmlns=\"http://lca.jrc.it/ILCD/Process\" xmlns:c=\"http://lca.jrc.it/ILCD/Contact\" xmlns:common=\"http://lca.jrc.it/ILCD/Common\" xmlns:epd=\"http://www.iai.kit.edu/EPD/2013\" xmlns:epd2=\"http://www.indata.network/EPD/2019\" xmlns:f=\"http://lca.jrc.it/ILCD/Flow\" xmlns:fp=\"http://lca.jrc.it/ILCD/FlowProperty\" xmlns:m=\"http://lca.jrc.it/ILCD/LCIAMethod\" xmlns:s=\"http://lca.jrc.it/ILCD/Source\" xmlns:u=\"http://lca.jrc.it/ILCD/UnitGroup\" name=\"C1\" scenario=\"Standard scenario\"/>", "<ns11:modules xmlns:ns11=\"http://openlca.org/epd_ilcd\" xmlns=\"http://lca.jrc.it/ILCD/Process\" xmlns:c=\"http://lca.jrc.it/ILCD/Contact\" xmlns:common=\"http://lca.jrc.it/ILCD/Common\" xmlns:epd=\"http://www.iai.kit.edu/EPD/2013\" xmlns:epd2=\"http://www.indata.network/EPD/2019\" xmlns:f=\"http://lca.jrc.it/ILCD/Flow\" xmlns:fp=\"http://lca.jrc.it/ILCD/FlowProperty\" xmlns:m=\"http://lca.jrc.it/ILCD/LCIAMethod\" xmlns:s=\"http://lca.jrc.it/ILCD/Source\" xmlns:u=\"http://lca.jrc.it/ILCD/UnitGroup\" name=\"C2\" scenario=\"Standard scenario\"/>", "<ns11:modules xmlns:ns11=\"http://openlca.org/epd_ilcd\" xmlns=\"http://lca.jrc.it/ILCD/Process\" xmlns:c=\"http://lca.jrc.it/ILCD/Contact\" xmlns:common=\"http://lca.jrc.it/ILCD/Common\" xmlns:epd=\"http://www.iai.kit.edu/EPD/2013\" xmlns:epd2=\"http://www.indata.network/EPD/2019\" xmlns:f=\"http://lca.jrc.it/ILCD/Flow\" xmlns:fp=\"http://lca.jrc.it/ILCD/FlowProperty\" xmlns:m=\"http://lca.jrc.it/ILCD/LCIAMethod\" xmlns:s=\"http://lca.jrc.it/ILCD/Source\" xmlns:u=\"http://lca.jrc.it/ILCD/UnitGroup\" name=\"C3\" scenario=\"Standard scenario\"/>", "<ns11:modules xmlns:ns11=\"http://openlca.org/epd_ilcd\" xmlns=\"http://lca.jrc.it/ILCD/Process\" xmlns:c=\"http://lca.jrc.it/ILCD/Contact\" xmlns:common=\"http://lca.jrc.it/ILCD/Common\" xmlns:epd=\"http://www.iai.kit.edu/EPD/2013\" xmlns:epd2=\"http://www.indata.network/EPD/2019\" xmlns:f=\"http://lca.jrc.it/ILCD/Flow\" xmlns:fp=\"http://lca.jrc.it/ILCD/FlowProperty\" xmlns:m=\"http://lca.jrc.it/ILCD/LCIAMethod\" xmlns:s=\"http://lca.jrc.it/ILCD/Source\" xmlns:u=\"http://lca.jrc.it/ILCD/UnitGroup\" name=\"C4\" scenario=\"Standard scenario\"/>", "<ns11:modules xmlns:ns11=\"http://openlca.org/epd_ilcd\" xmlns=\"http://lca.jrc.it/ILCD/Process\" xmlns:c=\"http://lca.jrc.it/ILCD/Contact\" xmlns:common=\"http://lca.jrc.it/ILCD/Common\" xmlns:epd=\"http://www.iai.kit.edu/EPD/2013\" xmlns:epd2=\"http://www.indata.network/EPD/2019\" xmlns:f=\"http://lca.jrc.it/ILCD/Flow\" xmlns:fp=\"http://lca.jrc.it/ILCD/FlowProperty\" xmlns:m=\"http://lca.jrc.it/ILCD/LCIAMethod\" xmlns:s=\"http://lca.jrc.it/ILCD/Source\" xmlns:u=\"http://lca.jrc.it/ILCD/UnitGroup\" name=\"D\" scenario=\"Standard scenario\"/>", {}]}}, "quantitativeReference": {"referenceToReferenceFlow": [1], "type": "Reference flow(s)"}, "time": {"referenceYear": 2021, "dataSetValidUntil": 2028, "timeRepresentativenessDescription": [{"value": "All product- and process-specific data were collected for the operating year 2021 and are therefore up-to-date", "lang": "en"}], "other": {"anies": [{"name": "publicationDateOfEPD", "value": 1700092800000}]}}, "geography": {"locationOfOperationSupplyOrProduction": {"descriptionOfRestrictions": [{"value": "The geographical reference area is Germany.", "lang": "en"}], "location": "DE"}}, "technology": {"technologyDescriptionAndIncludedProcesses": [{"value": "Secutex® Green is a 100% biodegradable, mechanically bonded nonwoven. Its biodegradability is certified, which means that residues of the product cause no harm to the environment. It is UV-resistant and can therefore be used in uncovered applications. It is a temporary solution, and vegetation and their roots take over the desired filter properties after its service life. No plastic is entered into the environment during the installation, operation, or renaturation of the product, and after its service life it can remain onsite or as composting after renaturation. Due to the industrial production of the fibres and the constant needling process, a continuous and reproducible quality of the nonwoven is ensured. This also ensure that the product can be assigned to a geotextile robustness class (GRK). The GRK (the abbreviation for the German word Geotextilerobustheitsklasse) is a German classification system to indicate the robustness of a nonwoven, and they are assigned to a geotextile robustness class according to their mass per unit area (gramage) in conjunction with the stamp penetration force. This classification is only used and recognized in Germany, so the product names without this behind it are used internationally (and will be used throughout this background report). The product is available in the robustness classes GRK 2 to GRK 5, and in widths of 2m, 4m, and 6m in standard. Variations from this are available on request (see also 3.1). Secutex® Green is available in the following standard grades: Secutex® Green 30G1 GRK 2 / Secutex® Green 30G1; Secutex® Green 40G1 GRK 3 / Secutex® Green 40G1; Secutex® Green 60G1 GRK 4 / Secutex® Green 60G1; Secutex® Green 90G1 GRK 5 / Secutex® Green 90G1; Secutex® Green120G1 GRK 5 / Secutex® Green 120G1.\r\nThe manufacturing location of Secutex® Green is Gewerbestr. 2, 32339 Espelkamp, Germany. The raw material is brought there, and the nonwoven is produced by carding and needle punching. Then, the product is packaged and internally transported into stock. Afterwards, the product is transported to the building site and installed there.\r\n", "lang": "en"}, {"value": "Secutex® Green ist ein 100 % biologisch abbaubares, mechanisch verfestigtes Vlies.\r\nSeine Biologischen Abbaubarkeit ist zertifiziert, was bedeutet, dass Rückstände des Produkts keine Umweltschäden verursachen. Es ist UV-beständig und kann daher auch in unbedeckten Anwendungen eingesetzt werden.\r\nEs handelt sich um eine temporäre Lösung, nach Ablauf der Nutzungsdauer übernehmen die Vegetation und deren Wurzeln die gewünschten Filterfunktionen.\r\nWährend der Installation, des Betriebs oder der Renaturierung gelangen keine Kunststoffe in die Umwelt. Nach Ende der Nutzungsdauer kann das Produkt vor Ort verbleiben oder kompostiert werden.\r\nDurch die industrielle Herstellung der Fasern und den konstanten Vernadelungsprozess wird eine gleichbleibende und reproduzierbare Qualität des Vlieses sichergestellt.\r\nDies ermöglicht auch die Zuordnung zu einer Geotextilenrobustheitsklasse (GRK).\r\nDie GRK ist ein deutsches Klassifizierungssystem, das die Robustheit eines Vliesstoffs anhand seiner Flächenmasse (g/m²) in Verbindung mit der Stempeldurchdrückkraft beschreibt.\r\nDiese Klassifizierung wird ausschließlich in Deutschland verwendet und anerkannt, weshalb Produktnamen ohne GRK-Angabe im internationalen Gebrauch verwendet werden (und auch in diesem Hintergrundbericht). Das Produkt ist in den Robustheitsklassen GRK 2 bis GRK 5 erhältlich sowie in Standardbreiten von 2 m, 4 m und 6 m. Abweichende Varianten sind auf Anfrage verfügbar (siehe auch Abschnitt 3.1).\r\nSecutex® Green ist in folgenden Standardausführungen erhältlich: Secutex® Green 30G1 GRK 2 / Secutex® Green 30G1; Secutex® Green 40G1 GRK 3 / Secutex® Green 40G1; Secutex® Green 60G1 GRK 4 / Secutex® Green 60G1; Secutex® Green 90G1 GRK 5 / Secutex® Green 90G1; Secutex® Green 120G1 GRK 5 / Secutex® Green 120G1.\r\nDer Produktionsstandort von Secutex® Green befindet sich in der Gewerbestraße 2, 32339 Espelkamp, Deutschland. Dorthin wird der Rohstoff geliefert, und das Vlies wird durch Krempeln und Vernadeln hergestellt. Anschließend wird das Produkt verpackt und intern eingelagert. Danach wird es zur Baustelle transportiert und dort eingebaut.\r\n", "lang": "de"}], "technologicalApplicability": [{"value": "Secutex® Green is, for example, suitable to protect soils, as erosion protection, for separating soils, and as a filter against unwanted soil particle transport. It can be used in the following fields of application (among others): Gardening and landscaping; Temporary road and path construction; Bank protection/natural watercourse development, coastal protection, and scour protection.", "lang": "en"}, {"value": "Secutex® Green eignet sich beispielsweise zum Schutz von Böden, als Erosionsschutz, zur Boden­trennung sowie als Filter gegen den unerwünschten Partikeltransport im Boden.\r\nEs kann unter anderem in folgenden Anwendungsbereichen eingesetzt werden: Garten- und Landschaftsbau; Temporärer Straßen- und Wegebau; Böschungssicherung, naturnahe Gewässerentwicklung, Küstenschutz und Auskolkungsschutz.\r\n", "lang": "de"}], "referenceToTechnologyFlowDiagrammOrPicture": [{"shortDescription": [{"value": "Flow chart Secutex® Green G1", "lang": "en"}], "type": "source data set", "refObjectId": "71235f1b-8243-4635-8d39-d3d7d3720e49", "version": "00.00.001"}]}}, "modellingAndValidation": {"LCIMethodAndAllocation": {"typeOfDataSet": "EPD", "referenceToLCAMethodDetails": [{"shortDescription": [{"value": "Kiwa-Ecobility Experts (Kiwa-EE) – Product Category Rules for Geosynthetic Products, EPD programme, Version 2, 2023-07-21", "lang": "en"}], "type": "source data set", "refObjectId": "17679d29-f6d6-42aa-929b-3c46de6f4145", "version": "00.00.001"}], "other": {"anies": [{"name": "subType", "value": "specific dataset"}]}}, "dataSourcesTreatmentAndRepresentativeness": {"referenceToDataSource": [{"shortDescription": [{"value": "ecoinvent 3.6 database", "lang": "en"}], "type": "source data set", "refObjectId": "766b9973-5ee8-48a2-8098-72c8e20b369f", "version": "00.00.001"}, {"shortDescription": [{"value": "ecoinvent database (general)", "lang": "en"}], "type": "source data set", "refObjectId": "b497a91f-e14b-4b69-8f28-f50eb1576766", "version": "00.03.002"}], "useAdviceForDataSet": [{"value": "Secutex® Green is, for example, suitable to protect soils, as erosion protection, for separating soils, and as a filter against unwanted soil particle transport. It can be used in the following fields of application (among others): Gardening and landscaping; Temporary road and path construction; Bank protection/natural watercourse development, coastal protection, and scour protection.", "lang": "en"}], "other": {"anies": [{"name": "referenceToOriginalEPD", "value": {"shortDescription": {"value": "Secutex® Green G1 EPD", "defaultValue": "Secutex® Green G1 EPD", "lstrings": [{"lang": "en", "value": "Secutex® Green G1 EPD"}]}, "version": {"version": 1, "majorVersion": 0, "minorVersion": 0, "subMinorVersion": 1, "zero": false, "versionString": "00.00.001"}, "type": "source data set", "uuid": {"uuid": "4241fa5f-0d63-4d32-9280-71f9dbfb0f58"}, "refObjectId": "4241fa5f-0d63-4d32-9280-71f9dbfb0f58", "versionAsString": "00.00.001", "resourceURLs": ["https://oekobaudat.de/OEKOBAU.DAT/resource/sources/4241fa5f-0d63-4d32-9280-71f9dbfb0f58/EPD-Kiwa-EE-000320-EN.pdf?version=00.00.001"]}}]}}, "validation": {"review": [{"reviewDetails": [{"value": "Independent verification of the declaration and data according to ISO 14025:2006.\r", "lang": "en"}], "referenceToNameOfReviewerAndInstitution": [{"shortDescription": [{"value": "Elisabet Amat Guasch (External verifier)", "lang": "en"}], "type": "contact data set", "refObjectId": "0b940721-b9a8-4b42-9aae-cba754debb32", "version": "00.00.001"}], "type": "Independent external review"}]}, "complianceDeclarations": {"compliance": [{"referenceToComplianceSystem": {"shortDescription": [{"value": "ISO 14025", "lang": "en"}], "type": "source data set", "refObjectId": "4f2eb655-6e44-4874-a95a-e28f5442cd4d", "version": "00.00.001"}}, {"referenceToComplianceSystem": {"shortDescription": [{"value": "EN 15804+A2 (EF 3.0)", "lang": "de"}, {"value": "EN 15804+A2 (EF 3.0)", "lang": "en"}], "type": "source data set", "refObjectId": "c0016b33-8cf7-415c-ac6e-deba0d21440d", "version": "00.02.000"}}]}}, "administrativeInformation": {"commissionerAndGoal": {"referenceToCommissioner": [{"shortDescription": [{"value": "Naue GmbH & Co. KG", "lang": "en"}], "type": "contact data set", "refObjectId": "07fd43bb-6057-49b9-8d3f-ee60e0f3e39a", "version": "00.00.001"}]}, "dataGenerator": {"referenceToPersonOrEntityGeneratingTheDataSet": [{"shortDescription": [{"value": "Kiwa GmbH (Berlin)", "lang": "en"}], "type": "contact data set", "refObjectId": "3ea4a87a-3f88-4633-b7e7-1bbdd272be43", "version": "00.00.002"}]}, "dataEntryBy": {"timeStamp": 1760451342189, "referenceToDataSetFormat": [{"shortDescription": [{"value": "EPD Data Format Extensions v1.2", "lang": "en"}, {"value": "EPD-Datenformaterweiterungen v1.2", "lang": "de"}], "type": "source data set", "refObjectId": "a29449fd-aa2f-4de8-b5d7-4b06b43c6fde", "version": "00.01.000"}, {"shortDescription": [{"value": "ILCD format", "lang": "en"}], "type": "source data set", "refObjectId": "a97a0155-0234-4b87-b4ce-a45da52f2a40", "version": "01.00.000", "uri": "http://lca.jrc.ec.europa.eu/lcainfohub/sample_data/ilcd/sources/ILCD_Format_a97a0155-0234-4b87-b4ce-a45da52f2a40_01.00.000.xml"}], "referenceToPersonOrEntityEnteringTheData": {"shortDescription": [{"value": "Kiwa-Ecobility Experts, Kiwa GmbH (Berlin)", "lang": "en"}], "type": "contact data set", "refObjectId": "eb52a9a8-9d0f-40ce-a5c9-7b78f5615e5a", "version": "00.00.002"}}, "publicationAndOwnership": {"dataSetVersion": "00.00.005", "referenceToRegistrationAuthority": {"shortDescription": [{"value": "Kiwa-Ecobility Experts, Kiwa GmbH (Berlin)", "lang": "en"}], "type": "contact data set", "refObjectId": "eb52a9a8-9d0f-40ce-a5c9-7b78f5615e5a", "version": "00.00.002"}, "registrationNumber": "EPD-Kiwa-EE-000320-EN", "referenceToOwnershipOfDataSet": {"shortDescription": [{"value": "Naue GmbH & Co. KG", "lang": "en"}], "type": "contact data set", "refObjectId": "07fd43bb-6057-49b9-8d3f-ee60e0f3e39a", "version": "00.00.001"}, "copyright": true, "licenseType": "Free of charge for all users and uses", "accessRestrictions": [{"value": "None.", "lang": "en"}], "other": {"anies": [{"name": "referenceToPublisher", "value": {"shortDescription": [{"value": "Kiwa-Ecobility Experts, Kiwa GmbH (Berlin)", "lang": "en"}], "type": "contact data set", "refObjectId": "eb52a9a8-9d0f-40ce-a5c9-7b78f5615e5a", "version": "00.00.002"}}]}}}, "exchanges": {"exchange": [{"dataSetInternalID": 1, "referenceToFlowDataSet": {"shortDescription": [{"value": "Secutex® Green G1", "lang": "en"}], "type": "flow data set", "refObjectId": "c752646d-0e4d-4ff6-b8cf-9abb22cd3533", "version": "00.00.003"}, "meanAmount": 1.0, "resultingAmount": 1.0, "referenceFlow": true, "resultingflowAmount": 1.0, "flowProperties": [{"name": [{"lang": "en", "value": "Carbon content (biogenic) - packaging"}], "uuid": "262a541b-209e-44cc-a426-33bce30de7b1", "meanValue": 0.0}, {"name": [{"lang": "de", "value": "Fläche"}, {"lang": "en", "value": "Area"}], "uuid": "93a60a56-a3c8-19da-a746-0800200c9a66", "referenceFlowProperty": true, "meanValue": 1.0, "referenceUnit": "qm", "unitGroupUUID": "c20a03d7-bd90-4569-bc94-66cfd364dfc8"}, {"name": [{"lang": "en", "value": "Carbon content (biogenic)"}], "uuid": "62e503ce-544a-4599-b2ad-bcea15a7bf20", "meanValue": 0.0}], "materialProperties": [{"name": "layer thickness", "value": "0.004", "unit": "m", "unitDescription": "meters"}, {"name": "grammage", "value": "0.6", "unit": "kg/m^2", "unitDescription": "kilograms per square meter"}], "typeOfFlow": "Product flow", "classification": {"classHierarchy": "Kunststoffe / Folien und Vliese / Technische Textilien", "name": "OEKOBAU.DAT"}}, {"dataSetInternalID": 2, "referenceToFlowDataSet": {"shortDescription": [{"value": "Components for re-use (CRU)", "lang": "en"}, {"value": "Komponenten für die Wiederverwendung (CRU)", "lang": "de"}, {"value": "Componentes para su reutilización (CRU)", "lang": "es"}], "type": "flow data set", "refObjectId": "a2b32f97-3fc7-4af2-b209-525bc6426f33", "version": "30.00.000", "uri": "../flows/a2b32f97-3fc7-4af2-b209-525bc6426f33.xml"}, "exchange direction": "OUTPUT", "meanAmount": 0.0, "other": {"anies": [{"value": "0.0", "module": "A1", "scenario": "Standard scenario"}, {"value": "0.0", "module": "A2", "scenario": "Standard scenario"}, {"value": "0.0", "module": "A3", "scenario": "Standard scenario"}, {"value": "0.0", "module": "C1", "scenario": "Standard scenario"}, {"value": "0.0", "module": "C2", "scenario": "Standard scenario"}, {"value": "0.0", "module": "C3", "scenario": "Standard scenario"}, {"value": "0.0", "module": "C4", "scenario": "Standard scenario"}, {"value": "0.0", "module": "D", "scenario": "Standard scenario"}, {"name": "referenceToUnitGroupDataSet", "value": {"shortDescription": [{"value": "kg", "lang": "en"}], "type": "unit group data set", "refObjectId": "ad38d542-3fe9-439d-9b95-2f5f7752acaf", "version": "30.00.000", "uri": "../unitgroups/ad38d542-3fe9-439d-9b95-2f5f7752acaf.xml"}}]}, "flowProperties": [], "typeOfFlow": "Other flow", "classification": {"classHierarchy": "Größen / Umweltliche Größen / EPD EN 15804 / LCI Indikatoren", "name": "GaBiCategories"}}, {"dataSetInternalID": 3, "referenceToFlowDataSet": {"shortDescription": [{"value": "Exported electrical energy (EEE)", "lang": "en"}, {"value": "Exportierte elektrische Energie (EEE)", "lang": "de"}, {"value": "Energía exportada electrica (EEE)", "lang": "es"}], "type": "flow data set", "refObjectId": "4da0c987-2b76-40d6-9e9e-82a017aaaf29", "version": "30.00.000", "uri": "../flows/4da0c987-2b76-40d6-9e9e-82a017aaaf29.xml"}, "exchange direction": "OUTPUT", "meanAmount": 0.0, "other": {"anies": [{"value": "0.0", "module": "A1", "scenario": "Standard scenario"}, {"value": "0.0", "module": "A2", "scenario": "Standard scenario"}, {"value": "1.5E-4", "module": "A3", "scenario": "Standard scenario"}, {"value": "0.0", "module": "C1", "scenario": "Standard scenario"}, {"value": "0.0", "module": "C2", "scenario": "Standard scenario"}, {"value": "0.0", "module": "C3", "scenario": "Standard scenario"}, {"value": "0.0", "module": "C4", "scenario": "Standard scenario"}, {"value": "0.0", "module": "D", "scenario": "Standard scenario"}, {"name": "referenceToUnitGroupDataSet", "value": {"shortDescription": [{"value": "MJ", "lang": "en"}], "type": "unit group data set", "refObjectId": "93a60a57-a3c8-11da-a746-0800200c9a66", "version": "03.00.000", "uri": "../unitgroups/93a60a57-a3c8-11da-a746-0800200c9a66.xml"}}]}, "flowProperties": [], "typeOfFlow": "Other flow", "classification": {"classHierarchy": "Größen / Umweltliche Größen / EPD EN 15804 / LCI Indikatoren", "name": "GaBiCategories"}}, {"dataSetInternalID": 4, "referenceToFlowDataSet": {"shortDescription": [{"value": "Exported thermal energy (EET)", "lang": "en"}, {"value": "Exportierte thermische Energie (EET)", "lang": "de"}, {"value": "Energía exportada termal (EET)", "lang": "es"}], "type": "flow data set", "refObjectId": "98daf38a-7a79-46d3-9a37-2b7bd0955810", "version": "30.00.000", "uri": "../flows/98daf38a-7a79-46d3-9a37-2b7bd0955810.xml"}, "exchange direction": "OUTPUT", "meanAmount": 0.0, "other": {"anies": [{"value": "0.0", "module": "A1", "scenario": "Standard scenario"}, {"value": "0.0", "module": "A2", "scenario": "Standard scenario"}, {"value": "2.58E-4", "module": "A3", "scenario": "Standard scenario"}, {"value": "0.0", "module": "C1", "scenario": "Standard scenario"}, {"value": "0.0", "module": "C2", "scenario": "Standard scenario"}, {"value": "0.0", "module": "C3", "scenario": "Standard scenario"}, {"value": "0.0", "module": "C4", "scenario": "Standard scenario"}, {"value": "0.0", "module": "D", "scenario": "Standard scenario"}, {"name": "referenceToUnitGroupDataSet", "value": {"shortDescription": [{"value": "MJ", "lang": "en"}], "type": "unit group data set", "refObjectId": "93a60a57-a3c8-11da-a746-0800200c9a66", "version": "03.00.000", "uri": "../unitgroups/93a60a57-a3c8-11da-a746-0800200c9a66.xml"}}]}, "flowProperties": [], "typeOfFlow": "Other flow", "classification": {"classHierarchy": "Größen / Umweltliche Größen / EPD EN 15804 / LCI Indikatoren", "name": "GaBiCategories"}}, {"dataSetInternalID": 5, "referenceToFlowDataSet": {"shortDescription": [{"value": "Use of net fresh water (FW)", "lang": "en"}, {"value": "Einsatz von Süßwasserressourcen (FW)", "lang": "de"}, {"value": "Uso neto de recursos de agua dulce (FW)", "lang": "es"}], "type": "flow data set", "refObjectId": "3cf952c8-f3a4-461d-8c96-96456ca62246", "version": "30.00.000", "uri": "../flows/3cf952c8-f3a4-461d-8c96-96456ca62246.xml"}, "exchange direction": "INPUT", "meanAmount": 0.0, "other": {"anies": [{"value": "0.0358", "module": "A1", "scenario": "Standard scenario"}, {"value": "1.18E-4", "module": "A2", "scenario": "Standard scenario"}, {"value": "0.00114", "module": "A3", "scenario": "Standard scenario"}, {"value": "0.0", "module": "C1", "scenario": "Standard scenario"}, {"value": "0.0", "module": "C2", "scenario": "Standard scenario"}, {"value": "0.0", "module": "C3", "scenario": "Standard scenario"}, {"value": "0.0", "module": "C4", "scenario": "Standard scenario"}, {"value": "0.0", "module": "D", "scenario": "Standard scenario"}, {"name": "referenceToUnitGroupDataSet", "value": {"shortDescription": [{"value": "m3", "lang": "en"}], "type": "unit group data set", "refObjectId": "cd950537-0a98-4044-9ba7-9f9a68d0a504", "version": "30.00.000", "uri": "../unitgroups/cd950537-0a98-4044-9ba7-9f9a68d0a504.xml"}}]}, "flowProperties": [], "typeOfFlow": "Other flow", "classification": {"classHierarchy": "Größen / Umweltliche Größen / EPD EN 15804 / LCI Indikatoren", "name": "GaBiCategories"}}, {"dataSetInternalID": 6, "referenceToFlowDataSet": {"shortDescription": [{"value": "Hazardous waste disposed (HWD)", "lang": "en"}, {"value": "Gefährlicher Abfall zur Deponie (HWD)", "lang": "de"}, {"value": "Residuos peligrosos eliminados (HWD)", "lang": "es"}], "type": "flow data set", "refObjectId": "430f9e0f-59b2-46a0-8e0d-55e0e84948fc", "version": "30.00.000", "uri": "../flows/430f9e0f-59b2-46a0-8e0d-55e0e84948fc.xml"}, "exchange direction": "OUTPUT", "meanAmount": 0.0, "other": {"anies": [{"value": "0.0", "module": "A1", "scenario": "Standard scenario"}, {"value": "2.45E-6", "module": "A2", "scenario": "Standard scenario"}, {"value": "8.07E-7", "module": "A3", "scenario": "Standard scenario"}, {"value": "0.0", "module": "C1", "scenario": "Standard scenario"}, {"value": "0.0", "module": "C2", "scenario": "Standard scenario"}, {"value": "0.0", "module": "C3", "scenario": "Standard scenario"}, {"value": "0.0", "module": "C4", "scenario": "Standard scenario"}, {"value": "0.0", "module": "D", "scenario": "Standard scenario"}, {"name": "referenceToUnitGroupDataSet", "value": {"shortDescription": [{"value": "kg", "lang": "en"}], "type": "unit group data set", "refObjectId": "ad38d542-3fe9-439d-9b95-2f5f7752acaf", "version": "30.00.000", "uri": "../unitgroups/ad38d542-3fe9-439d-9b95-2f5f7752acaf.xml"}}]}, "flowProperties": [], "typeOfFlow": "Other flow", "classification": {"classHierarchy": "Größen / Umweltliche Größen / EPD EN 15804 / LCI Indikatoren", "name": "GaBiCategories"}}, {"dataSetInternalID": 7, "referenceToFlowDataSet": {"shortDescription": [{"value": "Materials for energy recovery (MER)", "lang": "en"}, {"value": "Stoffe für die Energierückgewinnung (MER)", "lang": "de"}, {"value": "Materiales para valorización energética (recuperación de energía) (MER)", "lang": "es"}], "type": "flow data set", "refObjectId": "59a9181c-3aaf-46ee-8b13-2b3723b6e447", "version": "30.00.000", "uri": "../flows/59a9181c-3aaf-46ee-8b13-2b3723b6e447.xml"}, "exchange direction": "OUTPUT", "meanAmount": 0.0, "other": {"anies": [{"value": "0.0", "module": "A1", "scenario": "Standard scenario"}, {"value": "0.0", "module": "A2", "scenario": "Standard scenario"}, {"value": "0.0", "module": "A3", "scenario": "Standard scenario"}, {"value": "0.0", "module": "C1", "scenario": "Standard scenario"}, {"value": "0.0", "module": "C2", "scenario": "Standard scenario"}, {"value": "0.0", "module": "C3", "scenario": "Standard scenario"}, {"value": "0.0", "module": "C4", "scenario": "Standard scenario"}, {"value": "0.0", "module": "D", "scenario": "Standard scenario"}, {"name": "referenceToUnitGroupDataSet", "value": {"shortDescription": [{"value": "kg", "lang": "en"}], "type": "unit group data set", "refObjectId": "ad38d542-3fe9-439d-9b95-2f5f7752acaf", "version": "30.00.000", "uri": "../unitgroups/ad38d542-3fe9-439d-9b95-2f5f7752acaf.xml"}}]}, "flowProperties": [], "typeOfFlow": "Other flow", "classification": {"classHierarchy": "Größen / Umweltliche Größen / EPD EN 15804 / LCI Indikatoren", "name": "GaBiCategories"}}, {"dataSetInternalID": 8, "referenceToFlowDataSet": {"shortDescription": [{"value": "Materials for recycling (MFR)", "lang": "en"}, {"value": "Stoffe zum Recycling (MFR)", "lang": "de"}, {"value": "Materiales para el reciclaje (MFR)", "lang": "es"}], "type": "flow data set", "refObjectId": "d7fe48a5-4103-49c8-9aae-b0b5dfdbd6ae", "version": "30.00.000", "uri": "../flows/d7fe48a5-4103-49c8-9aae-b0b5dfdbd6ae.xml"}, "exchange direction": "OUTPUT", "meanAmount": 0.0, "other": {"anies": [{"value": "0.0", "module": "A1", "scenario": "Standard scenario"}, {"value": "0.0", "module": "A2", "scenario": "Standard scenario"}, {"value": "0.0", "module": "A3", "scenario": "Standard scenario"}, {"value": "0.0", "module": "C1", "scenario": "Standard scenario"}, {"value": "0.0", "module": "C2", "scenario": "Standard scenario"}, {"value": "0.0", "module": "C3", "scenario": "Standard scenario"}, {"value": "0.0", "module": "C4", "scenario": "Standard scenario"}, {"value": "0.0", "module": "D", "scenario": "Standard scenario"}, {"name": "referenceToUnitGroupDataSet", "value": {"shortDescription": [{"value": "kg", "lang": "en"}], "type": "unit group data set", "refObjectId": "ad38d542-3fe9-439d-9b95-2f5f7752acaf", "version": "30.00.000", "uri": "../unitgroups/ad38d542-3fe9-439d-9b95-2f5f7752acaf.xml"}}]}, "flowProperties": [], "typeOfFlow": "Other flow", "classification": {"classHierarchy": "Größen / Umweltliche Größen / EPD EN 15804 / LCI Indikatoren", "name": "GaBiCategories"}}, {"dataSetInternalID": 9, "referenceToFlowDataSet": {"shortDescription": [{"value": "Non-hazardous waste disposed (NHWD)", "lang": "en"}, {"value": "Entsorgter nicht gefährlicher Abfall (NHWD)", "lang": "de"}, {"value": "Residuos no peligrosos eliminados (NHWD)", "lang": "es"}], "type": "flow data set", "refObjectId": "b29ef66b-e286-4afa-949f-62f1a7b4d7fa", "version": "30.00.000", "uri": "../flows/b29ef66b-e286-4afa-949f-62f1a7b4d7fa.xml"}, "exchange direction": "OUTPUT", "meanAmount": 0.0, "other": {"anies": [{"value": "0.0", "module": "A1", "scenario": "Standard scenario"}, {"value": "0.0614", "module": "A2", "scenario": "Standard scenario"}, {"value": "0.00963", "module": "A3", "scenario": "Standard scenario"}, {"value": "0.0", "module": "C1", "scenario": "Standard scenario"}, {"value": "0.0", "module": "C2", "scenario": "Standard scenario"}, {"value": "0.0", "module": "C3", "scenario": "Standard scenario"}, {"value": "0.0", "module": "C4", "scenario": "Standard scenario"}, {"value": "0.0", "module": "D", "scenario": "Standard scenario"}, {"name": "referenceToUnitGroupDataSet", "value": {"shortDescription": [{"value": "kg", "lang": "en"}], "type": "unit group data set", "refObjectId": "ad38d542-3fe9-439d-9b95-2f5f7752acaf", "version": "30.00.000", "uri": "../unitgroups/ad38d542-3fe9-439d-9b95-2f5f7752acaf.xml"}}]}, "flowProperties": [], "typeOfFlow": "Other flow", "classification": {"classHierarchy": "Größen / Umweltliche Größen / EPD EN 15804 / LCI Indikatoren", "name": "GaBiCategories"}}, {"dataSetInternalID": 10, "referenceToFlowDataSet": {"shortDescription": [{"value": "Use of non renewable secondary fuels (NRSF)", "lang": "en"}, {"value": "Nicht erneuerbare Sekundärbrennstoffe (NRSF)", "lang": "de"}, {"value": "Uso de combustibles secundarios no renovables (NRSF)", "lang": "es"}], "type": "flow data set", "refObjectId": "89def144-d39a-4287-b86f-efde453ddcb2", "version": "30.00.000", "uri": "../flows/89def144-d39a-4287-b86f-efde453ddcb2.xml"}, "exchange direction": "INPUT", "meanAmount": 0.0, "other": {"anies": [{"value": "0.0", "module": "A1", "scenario": "Standard scenario"}, {"value": "0.0", "module": "A2", "scenario": "Standard scenario"}, {"value": "0.0", "module": "A3", "scenario": "Standard scenario"}, {"value": "0.0", "module": "C1", "scenario": "Standard scenario"}, {"value": "0.0", "module": "C2", "scenario": "Standard scenario"}, {"value": "0.0", "module": "C3", "scenario": "Standard scenario"}, {"value": "0.0", "module": "C4", "scenario": "Standard scenario"}, {"value": "0.0", "module": "D", "scenario": "Standard scenario"}, {"name": "referenceToUnitGroupDataSet", "value": {"shortDescription": [{"value": "MJ", "lang": "en"}], "type": "unit group data set", "refObjectId": "93a60a57-a3c8-11da-a746-0800200c9a66", "version": "03.00.000", "uri": "../unitgroups/93a60a57-a3c8-11da-a746-0800200c9a66.xml"}}]}, "flowProperties": [], "typeOfFlow": "Other flow", "classification": {"classHierarchy": "Größen / Umweltliche Größen / EPD EN 15804 / LCI Indikatoren", "name": "GaBiCategories"}}, {"dataSetInternalID": 11, "referenceToFlowDataSet": {"shortDescription": [{"value": "Use of non renewable primary energy (PENRE)", "lang": "en"}, {"value": "Nicht-erneuerbare Primärenergie als Energieträger (PENRE)", "lang": "de"}, {"value": "Uso de energía primaria no renovable, excluyendo los recursos de energía primaria no renovable utilizada como materia prima (PENRE)", "lang": "es"}], "type": "flow data set", "refObjectId": "ac857178-2b45-46ec-892a-a9a4332f0372", "version": "38.00.000", "uri": "../flows/ac857178-2b45-46ec-892a-a9a4332f0372.xml"}, "exchange direction": "INPUT", "meanAmount": 0.0, "other": {"anies": [{"value": "0.0", "module": "A1", "scenario": "Standard scenario"}, {"value": "1.03", "module": "A2", "scenario": "Standard scenario"}, {"value": "0.401", "module": "A3", "scenario": "Standard scenario"}, {"value": "0.0", "module": "C1", "scenario": "Standard scenario"}, {"value": "0.0", "module": "C2", "scenario": "Standard scenario"}, {"value": "0.0", "module": "C3", "scenario": "Standard scenario"}, {"value": "0.0", "module": "C4", "scenario": "Standard scenario"}, {"value": "0.0", "module": "D", "scenario": "Standard scenario"}, {"name": "referenceToUnitGroupDataSet", "value": {"shortDescription": [{"value": "MJ", "lang": "en"}], "type": "unit group data set", "refObjectId": "93a60a57-a3c8-11da-a746-0800200c9a66", "version": "03.00.000", "uri": "../unitgroups/93a60a57-a3c8-11da-a746-0800200c9a66.xml"}}]}, "flowProperties": [], "typeOfFlow": "Other flow", "classification": {"classHierarchy": "Quantities", "name": "GaBiCategories"}}, {"dataSetInternalID": 12, "referenceToFlowDataSet": {"shortDescription": [{"value": "Use of non renewable primary energy resources used as raw materials (PENRM)", "lang": "en"}, {"value": "Nicht-erneuerbare Primärenergie zur stofflichen Nutzung (PENRM)", "lang": "de"}, {"value": "Uso de la energía primaria no renovable utilizada como materia prima (PENRM)", "lang": "es"}], "type": "flow data set", "refObjectId": "1421caa0-679d-4bf4-b282-0eb850ccae27", "version": "38.00.000", "uri": "../flows/1421caa0-679d-4bf4-b282-0eb850ccae27.xml"}, "exchange direction": "INPUT", "meanAmount": 0.0, "other": {"anies": [{"value": "0.0", "module": "A1", "scenario": "Standard scenario"}, {"value": "0.0", "module": "A2", "scenario": "Standard scenario"}, {"value": "0.213", "module": "A3", "scenario": "Standard scenario"}, {"value": "0.0", "module": "C1", "scenario": "Standard scenario"}, {"value": "0.0", "module": "C2", "scenario": "Standard scenario"}, {"value": "0.0", "module": "C3", "scenario": "Standard scenario"}, {"value": "0.0", "module": "C4", "scenario": "Standard scenario"}, {"value": "0.0", "module": "D", "scenario": "Standard scenario"}, {"name": "referenceToUnitGroupDataSet", "value": {"shortDescription": [{"value": "MJ", "lang": "en"}], "type": "unit group data set", "refObjectId": "93a60a57-a3c8-11da-a746-0800200c9a66", "version": "03.00.000", "uri": "../unitgroups/93a60a57-a3c8-11da-a746-0800200c9a66.xml"}}]}, "flowProperties": [], "typeOfFlow": "Other flow", "classification": {"classHierarchy": "Quantities", "name": "GaBiCategories"}}, {"dataSetInternalID": 13, "referenceToFlowDataSet": {"shortDescription": [{"value": "Total use of non-renewable primary energy resources (PENRT)", "lang": "en"}, {"value": "Total nicht erneuerbare Primärenergie (PENRT)", "lang": "de"}, {"value": "Uso total de la energía primaria no renovable (energía primaria y recursos de energía primaria renovable utilizada como materia prima) (PENRT)", "lang": "es"}], "type": "flow data set", "refObjectId": "06159210-646b-4c8d-8583-da9b3b95a6c1", "version": "30.00.000", "uri": "../flows/06159210-646b-4c8d-8583-da9b3b95a6c1.xml"}, "exchange direction": "INPUT", "meanAmount": 0.0, "other": {"anies": [{"value": "0.0", "module": "A1", "scenario": "Standard scenario"}, {"value": "1.03", "module": "A2", "scenario": "Standard scenario"}, {"value": "0.613", "module": "A3", "scenario": "Standard scenario"}, {"value": "0.0", "module": "C1", "scenario": "Standard scenario"}, {"value": "0.0", "module": "C2", "scenario": "Standard scenario"}, {"value": "0.0", "module": "C3", "scenario": "Standard scenario"}, {"value": "0.0", "module": "C4", "scenario": "Standard scenario"}, {"value": "0.0", "module": "D", "scenario": "Standard scenario"}, {"name": "referenceToUnitGroupDataSet", "value": {"shortDescription": [{"value": "MJ", "lang": "en"}], "type": "unit group data set", "refObjectId": "93a60a57-a3c8-11da-a746-0800200c9a66", "version": "03.00.000", "uri": "../unitgroups/93a60a57-a3c8-11da-a746-0800200c9a66.xml"}}]}, "flowProperties": [], "typeOfFlow": "Other flow", "classification": {"classHierarchy": "Größen / Umweltliche Größen / EPD EN 15804 / LCI Indikatoren", "name": "GaBiCategories"}}, {"dataSetInternalID": 14, "referenceToFlowDataSet": {"shortDescription": [{"value": "Use of renewable primary energy (PERE)", "lang": "en"}, {"value": "Erneuerbare Primärenergie als Energieträger (PERE)", "lang": "de"}, {"value": "Uso de energía primaria renovable excluyendo los recursos de energía primaria renovable utilizada como materia prima (PERE)", "lang": "es"}], "type": "flow data set", "refObjectId": "20f32be5-0398-4288-9b6d-accddd195317", "version": "38.00.000", "uri": "../flows/20f32be5-0398-4288-9b6d-accddd195317.xml"}, "exchange direction": "INPUT", "meanAmount": 0.0, "other": {"anies": [{"value": "0.0", "module": "A1", "scenario": "Standard scenario"}, {"value": "0.0121", "module": "A2", "scenario": "Standard scenario"}, {"value": "0.353", "module": "A3", "scenario": "Standard scenario"}, {"value": "0.0", "module": "C1", "scenario": "Standard scenario"}, {"value": "0.0", "module": "C2", "scenario": "Standard scenario"}, {"value": "0.0", "module": "C3", "scenario": "Standard scenario"}, {"value": "0.0", "module": "C4", "scenario": "Standard scenario"}, {"value": "0.0", "module": "D", "scenario": "Standard scenario"}, {"name": "referenceToUnitGroupDataSet", "value": {"shortDescription": [{"value": "MJ", "lang": "en"}], "type": "unit group data set", "refObjectId": "93a60a57-a3c8-11da-a746-0800200c9a66", "version": "03.00.000", "uri": "../unitgroups/93a60a57-a3c8-11da-a746-0800200c9a66.xml"}}]}, "flowProperties": [], "typeOfFlow": "Other flow", "classification": {"classHierarchy": "Quantities", "name": "GaBiCategories"}}, {"dataSetInternalID": 15, "referenceToFlowDataSet": {"shortDescription": [{"value": "Use of renewable primary energy resources used as raw materials (PERM)", "lang": "en"}, {"value": "Erneuerbare Primärenergie zur stofflichen Nutzung (PERM)", "lang": "de"}, {"value": "Uso de energía primaria renovable utilizada como materia prima (PERM)", "lang": "es"}], "type": "flow data set", "refObjectId": "fb3ec0de-548d-4508-aea5-00b73bf6f702", "version": "38.00.000", "uri": "../flows/fb3ec0de-548d-4508-aea5-00b73bf6f702.xml"}, "exchange direction": "INPUT", "meanAmount": 0.0, "other": {"anies": [{"value": "0.0", "module": "A1", "scenario": "Standard scenario"}, {"value": "0.0", "module": "A2", "scenario": "Standard scenario"}, {"value": "0.611", "module": "A3", "scenario": "Standard scenario"}, {"value": "0.0", "module": "C1", "scenario": "Standard scenario"}, {"value": "0.0", "module": "C2", "scenario": "Standard scenario"}, {"value": "0.0", "module": "C3", "scenario": "Standard scenario"}, {"value": "0.0", "module": "C4", "scenario": "Standard scenario"}, {"value": "0.0", "module": "D", "scenario": "Standard scenario"}, {"name": "referenceToUnitGroupDataSet", "value": {"shortDescription": [{"value": "MJ", "lang": "en"}], "type": "unit group data set", "refObjectId": "93a60a57-a3c8-11da-a746-0800200c9a66", "version": "03.00.000", "uri": "../unitgroups/93a60a57-a3c8-11da-a746-0800200c9a66.xml"}}]}, "flowProperties": [], "typeOfFlow": "Other flow", "classification": {"classHierarchy": "Quantities", "name": "GaBiCategories"}}, {"dataSetInternalID": 16, "referenceToFlowDataSet": {"shortDescription": [{"value": "Total use of renewable primary energy resources (PERT)", "lang": "en"}, {"value": "Total erneuerbare Primärenergie (PERT)", "lang": "de"}, {"value": "Uso total de la energía primaria renovable (energía primaria y recursos de energía primaria renovable utilizada como materia prima) (PERT)", "lang": "es"}], "type": "flow data set", "refObjectId": "53f97275-fa8a-4cdd-9024-65936002acd0", "version": "30.00.000", "uri": "../flows/53f97275-fa8a-4cdd-9024-65936002acd0.xml"}, "exchange direction": "INPUT", "meanAmount": 0.0, "other": {"anies": [{"value": "0.0", "module": "A1", "scenario": "Standard scenario"}, {"value": "0.0121", "module": "A2", "scenario": "Standard scenario"}, {"value": "0.964", "module": "A3", "scenario": "Standard scenario"}, {"value": "0.0", "module": "C1", "scenario": "Standard scenario"}, {"value": "0.0", "module": "C2", "scenario": "Standard scenario"}, {"value": "0.0", "module": "C3", "scenario": "Standard scenario"}, {"value": "0.0", "module": "C4", "scenario": "Standard scenario"}, {"value": "0.0", "module": "D", "scenario": "Standard scenario"}, {"name": "referenceToUnitGroupDataSet", "value": {"shortDescription": [{"value": "MJ", "lang": "en"}], "type": "unit group data set", "refObjectId": "93a60a57-a3c8-11da-a746-0800200c9a66", "version": "03.00.000", "uri": "../unitgroups/93a60a57-a3c8-11da-a746-0800200c9a66.xml"}}]}, "flowProperties": [], "typeOfFlow": "Other flow", "classification": {"classHierarchy": "Größen / Umweltliche Größen / EPD EN 15804 / LCI Indikatoren", "name": "GaBiCategories"}}, {"dataSetInternalID": 17, "referenceToFlowDataSet": {"shortDescription": [{"value": "Use of renewable secondary fuels (RSF)", "lang": "en"}, {"value": "Erneuerbare Sekundärbrennstoffe (RSF)", "lang": "de"}, {"value": "Uso de combustibles secundarios renovables (RSF)", "lang": "es"}], "type": "flow data set", "refObjectId": "64333088-a55f-4aa2-9a31-c10b07816787", "version": "30.00.000", "uri": "../flows/64333088-a55f-4aa2-9a31-c10b07816787.xml"}, "exchange direction": "INPUT", "meanAmount": 0.0, "other": {"anies": [{"value": "0.0", "module": "A1", "scenario": "Standard scenario"}, {"value": "0.0", "module": "A2", "scenario": "Standard scenario"}, {"value": "0.0", "module": "A3", "scenario": "Standard scenario"}, {"value": "0.0", "module": "C1", "scenario": "Standard scenario"}, {"value": "0.0", "module": "C2", "scenario": "Standard scenario"}, {"value": "0.0", "module": "C3", "scenario": "Standard scenario"}, {"value": "0.0", "module": "C4", "scenario": "Standard scenario"}, {"value": "0.0", "module": "D", "scenario": "Standard scenario"}, {"name": "referenceToUnitGroupDataSet", "value": {"shortDescription": [{"value": "MJ", "lang": "en"}], "type": "unit group data set", "refObjectId": "93a60a57-a3c8-11da-a746-0800200c9a66", "version": "03.00.000", "uri": "../unitgroups/93a60a57-a3c8-11da-a746-0800200c9a66.xml"}}]}, "flowProperties": [], "typeOfFlow": "Other flow", "classification": {"classHierarchy": "Größen / Umweltliche Größen / EPD EN 15804 / LCI Indikatoren", "name": "GaBiCategories"}}, {"dataSetInternalID": 18, "referenceToFlowDataSet": {"shortDescription": [{"value": "Radioactive waste disposed (RWD)", "lang": "en"}, {"value": "Entsorgter radioaktiver Abfall (RWD)", "lang": "de"}, {"value": "Residuos radiactivos eliminados (RWD)", "lang": "es"}], "type": "flow data set", "refObjectId": "3449546e-52ad-4b39-b809-9fb77cea8ff6", "version": "30.00.000", "uri": "../flows/3449546e-52ad-4b39-b809-9fb77cea8ff6.xml"}, "exchange direction": "OUTPUT", "meanAmount": 0.0, "other": {"anies": [{"value": "0.0", "module": "A1", "scenario": "Standard scenario"}, {"value": "6.35E-6", "module": "A2", "scenario": "Standard scenario"}, {"value": "2.67E-6", "module": "A3", "scenario": "Standard scenario"}, {"value": "0.0", "module": "C1", "scenario": "Standard scenario"}, {"value": "0.0", "module": "C2", "scenario": "Standard scenario"}, {"value": "0.0", "module": "C3", "scenario": "Standard scenario"}, {"value": "0.0", "module": "C4", "scenario": "Standard scenario"}, {"value": "0.0", "module": "D", "scenario": "Standard scenario"}, {"name": "referenceToUnitGroupDataSet", "value": {"shortDescription": [{"value": "kg", "lang": "en"}], "type": "unit group data set", "refObjectId": "ad38d542-3fe9-439d-9b95-2f5f7752acaf", "version": "30.00.000", "uri": "../unitgroups/ad38d542-3fe9-439d-9b95-2f5f7752acaf.xml"}}]}, "flowProperties": [], "typeOfFlow": "Other flow", "classification": {"classHierarchy": "Größen / Umweltliche Größen / EPD EN 15804 / LCI Indikatoren", "name": "GaBiCategories"}}, {"dataSetInternalID": 19, "referenceToFlowDataSet": {"shortDescription": [{"value": "Use of secondary material (SM)", "lang": "en"}, {"value": "Einsatz von Sekundärstoffen (SM)", "lang": "de"}, {"value": "Uso de materiales secundarios (SM)", "lang": "es"}], "type": "flow data set", "refObjectId": "c6a1f35f-2d09-4f54-8dfb-97e502e1ce92", "version": "30.00.000", "uri": "../flows/c6a1f35f-2d09-4f54-8dfb-97e502e1ce92.xml"}, "exchange direction": "INPUT", "meanAmount": 0.0, "other": {"anies": [{"value": "0.0", "module": "A1", "scenario": "Standard scenario"}, {"value": "0.0", "module": "A2", "scenario": "Standard scenario"}, {"value": "0.043", "module": "A3", "scenario": "Standard scenario"}, {"value": "0.0", "module": "C1", "scenario": "Standard scenario"}, {"value": "0.0", "module": "C2", "scenario": "Standard scenario"}, {"value": "0.0", "module": "C3", "scenario": "Standard scenario"}, {"value": "0.0", "module": "C4", "scenario": "Standard scenario"}, {"value": "0.0", "module": "D", "scenario": "Standard scenario"}, {"name": "referenceToUnitGroupDataSet", "value": {"shortDescription": [{"value": "kg", "lang": "en"}], "type": "unit group data set", "refObjectId": "ad38d542-3fe9-439d-9b95-2f5f7752acaf", "version": "30.00.000", "uri": "../unitgroups/ad38d542-3fe9-439d-9b95-2f5f7752acaf.xml"}}]}, "flowProperties": [], "typeOfFlow": "Other flow", "classification": {"classHierarchy": "Größen / Umweltliche Größen / EPD EN 15804 / LCI Indikatoren", "name": "GaBiCategories"}}]}, "LCIAResults": {"LCIAResult": [{"referenceToLCIAMethodDataSet": {"shortDescription": [{"value": "Abiotic depletion potential - non-fossil resources (ADPE)", "lang": "en"}, {"value": "Potenzial für die Verknappung abiotischer Ressourcen – nicht fossile Ressourcen (ADPE)", "lang": "de"}], "type": "LCIA method data set", "refObjectId": "b2ad6494-c78d-11e6-9d9d-cec0c932ce01", "version": "01.00.011", "uri": "../lciamethods/b2ad6494-c78d-11e6-9d9d-cec0c932ce01.xml"}, "meanAmount": 0.0, "other": {"anies": [{"value": "9.88E-7", "module": "A1", "scenario": "Standard scenario"}, {"value": "1.63E-6", "module": "A2", "scenario": "Standard scenario"}, {"value": "5.18E-7", "module": "A3", "scenario": "Standard scenario"}, {"value": "0.0", "module": "C1", "scenario": "Standard scenario"}, {"value": "0.0", "module": "C2", "scenario": "Standard scenario"}, {"value": "0.0", "module": "C3", "scenario": "Standard scenario"}, {"value": "0.0", "module": "C4", "scenario": "Standard scenario"}, {"value": "0.0", "module": "D", "scenario": "Standard scenario"}, {"name": "referenceToUnitGroupDataSet", "value": {"shortDescription": [{"value": "kg Sb-eq.", "lang": "en"}], "type": "unit group data set", "refObjectId": "54ccd2d9-a32a-4fc2-923d-f2c8c93e89d4", "version": "30.00.000", "uri": "../unitgroups/54ccd2d9-a32a-4fc2-923d-f2c8c93e89d4.xml"}}]}}, {"referenceToLCIAMethodDataSet": {"shortDescription": [{"value": "Abiotic depletion potential - fossil resources (ADPF)", "lang": "en"}, {"value": "Potenzial für die Verknappung abiotischer Ressourcen – fossile Brennstoffe (ADPF)", "lang": "de"}], "type": "LCIA method data set", "refObjectId": "b2ad6110-c78d-11e6-9d9d-cec0c932ce01", "version": "01.00.011", "uri": "../lciamethods/b2ad6110-c78d-11e6-9d9d-cec0c932ce01.xml"}, "meanAmount": 0.0, "other": {"anies": [{"value": "30.7", "module": "A1", "scenario": "Standard scenario"}, {"value": "0.968", "module": "A2", "scenario": "Standard scenario"}, {"value": "1.19", "module": "A3", "scenario": "Standard scenario"}, {"value": "0.0", "module": "C1", "scenario": "Standard scenario"}, {"value": "0.0", "module": "C2", "scenario": "Standard scenario"}, {"value": "0.0", "module": "C3", "scenario": "Standard scenario"}, {"value": "0.0", "module": "C4", "scenario": "Standard scenario"}, {"value": "0.0", "module": "D", "scenario": "Standard scenario"}, {"name": "referenceToUnitGroupDataSet", "value": {"shortDescription": [{"value": "MJ", "lang": "en"}], "type": "unit group data set", "refObjectId": "93a60a57-a3c8-11da-a746-0800200c9a66", "version": "03.00.000", "uri": "../unitgroups/93a60a57-a3c8-11da-a746-0800200c9a66.xml"}}]}}, {"referenceToLCIAMethodDataSet": {"shortDescription": [{"value": "Acidification potential, Accumulated Exceedance (AP)", "lang": "en"}, {"value": "Versauerungspotenzial, kumulierte Überschreitung (AP)", "lang": "de"}], "type": "LCIA method data set", "refObjectId": "b5c611c6-def3-11e6-bf01-fe55135034f3", "version": "01.03.010", "uri": "../lciamethods/b5c611c6-def3-11e6-bf01-fe55135034f3.xml"}, "meanAmount": 0.0, "other": {"anies": [{"value": "0.012", "module": "A1", "scenario": "Standard scenario"}, {"value": "3.72E-4", "module": "A2", "scenario": "Standard scenario"}, {"value": "4.71E-4", "module": "A3", "scenario": "Standard scenario"}, {"value": "0.0", "module": "C1", "scenario": "Standard scenario"}, {"value": "0.0", "module": "C2", "scenario": "Standard scenario"}, {"value": "0.0", "module": "C3", "scenario": "Standard scenario"}, {"value": "0.0", "module": "C4", "scenario": "Standard scenario"}, {"value": "0.0", "module": "D", "scenario": "Standard scenario"}, {"name": "referenceToUnitGroupDataSet", "value": {"shortDescription": [{"value": "mol H+-eq.", "lang": "en"}], "type": "unit group data set", "refObjectId": "42e089ac-92bf-4bf2-8ca1-5fc40d18f2ed", "version": "00.01.000", "uri": "../unitgroups/42e089ac-92bf-4bf2-8ca1-5fc40d18f2ed.xml"}}]}}, {"referenceToLCIAMethodDataSet": {"shortDescription": [{"value": "Eutrophication potential - freshwater (EP-freshwater)", "lang": "en"}, {"value": "Eutrophierungspotenzial - Süßwasser (EP-freshwater)", "lang": "de"}], "type": "LCIA method data set", "refObjectId": "b53ec18f-7377-4ad3-86eb-cc3f4f276b2b", "version": "01.00.011", "uri": "../lciamethods/b53ec18f-7377-4ad3-86eb-cc3f4f276b2b.xml"}, "meanAmount": 0.0, "other": {"anies": [{"value": "1.37E-4", "module": "A1", "scenario": "Standard scenario"}, {"value": "6.47E-7", "module": "A2", "scenario": "Standard scenario"}, {"value": "6.02E-6", "module": "A3", "scenario": "Standard scenario"}, {"value": "0.0", "module": "C1", "scenario": "Standard scenario"}, {"value": "0.0", "module": "C2", "scenario": "Standard scenario"}, {"value": "0.0", "module": "C3", "scenario": "Standard scenario"}, {"value": "0.0", "module": "C4", "scenario": "Standard scenario"}, {"value": "0.0", "module": "D", "scenario": "Standard scenario"}, {"name": "referenceToUnitGroupDataSet", "value": {"shortDescription": [{"value": "kg P-eq.", "lang": "en"}], "type": "unit group data set", "refObjectId": "0429039d-a61d-4590-ba67-aa4a20a810a1", "version": "30.00.000", "uri": "../unitgroups/0429039d-a61d-4590-ba67-aa4a20a810a1.xml"}}]}}, {"referenceToLCIAMethodDataSet": {"shortDescription": [{"value": "Eutrophication potential - marine (EP-marine)", "lang": "en"}, {"value": "Eutrophierungspotenzial - Salzwasser (EP-marine)", "lang": "de"}], "type": "LCIA method data set", "refObjectId": "b5c619fa-def3-11e6-bf01-fe55135034f3", "version": "02.00.011", "uri": "../lciamethods/b5c619fa-def3-11e6-bf01-fe55135034f3.xml"}, "meanAmount": 0.0, "other": {"anies": [{"value": "0.00231", "module": "A1", "scenario": "Standard scenario"}, {"value": "1.31E-4", "module": "A2", "scenario": "Standard scenario"}, {"value": "9.94E-5", "module": "A3", "scenario": "Standard scenario"}, {"value": "0.0", "module": "C1", "scenario": "Standard scenario"}, {"value": "0.0", "module": "C2", "scenario": "Standard scenario"}, {"value": "0.0", "module": "C3", "scenario": "Standard scenario"}, {"value": "0.0", "module": "C4", "scenario": "Standard scenario"}, {"value": "0.0", "module": "D", "scenario": "Standard scenario"}, {"name": "referenceToUnitGroupDataSet", "value": {"shortDescription": [{"value": "kg N-eq.", "lang": "en"}], "type": "unit group data set", "refObjectId": "d05bb823-ecdf-4686-8c40-bf1d9257859f", "version": "00.00.003", "uri": "../unitgroups/d05bb823-ecdf-4686-8c40-bf1d9257859f.xml"}}]}}, {"referenceToLCIAMethodDataSet": {"shortDescription": [{"value": "Eutrophication potential - terrestrial (EP-terrestrial)", "lang": "en"}, {"value": "Eutrophierungspotenzial - Land (EP-terrestrial)", "lang": "de"}], "type": "LCIA method data set", "refObjectId": "b5c614d2-def3-11e6-bf01-fe55135034f3", "version": "01.02.010", "uri": "../lciamethods/b5c614d2-def3-11e6-bf01-fe55135034f3.xml"}, "meanAmount": 0.0, "other": {"anies": [{"value": "0.0244", "module": "A1", "scenario": "Standard scenario"}, {"value": "0.00145", "module": "A2", "scenario": "Standard scenario"}, {"value": "0.00119", "module": "A3", "scenario": "Standard scenario"}, {"value": "0.0", "module": "C1", "scenario": "Standard scenario"}, {"value": "0.0", "module": "C2", "scenario": "Standard scenario"}, {"value": "0.0", "module": "C3", "scenario": "Standard scenario"}, {"value": "0.0", "module": "C4", "scenario": "Standard scenario"}, {"value": "0.0", "module": "D", "scenario": "Standard scenario"}, {"name": "referenceToUnitGroupDataSet", "value": {"shortDescription": [{"value": "mol N-eq.", "lang": "en"}], "type": "unit group data set", "refObjectId": "71b4d617-0ec9-4d3f-b65e-e438940c2401", "version": "00.00.003", "uri": "../unitgroups/71b4d617-0ec9-4d3f-b65e-e438940c2401.xml"}}]}}, {"referenceToLCIAMethodDataSet": {"shortDescription": [{"value": "Potential Comparative Toxic Unit for ecosystems (ETP-fw)", "lang": "en"}, {"value": "Potenzielle Toxizitätsvergleichseinheit für Ökosysteme (ETP-fw)", "lang": "de"}], "type": "LCIA method data set", "refObjectId": "ee1082d1-b0f7-43ca-a1f0-21e2a4a74511", "version": "01.00.003", "uri": "../lciamethods/ee1082d1-b0f7-43ca-a1f0-21e2a4a74511.xml"}, "meanAmount": 0.0, "other": {"anies": [{"value": "0.871", "module": "A1", "scenario": "Standard scenario"}, {"value": "0.863", "module": "A2", "scenario": "Standard scenario"}, {"value": "1.77", "module": "A3", "scenario": "Standard scenario"}, {"value": "0.0", "module": "C1", "scenario": "Standard scenario"}, {"value": "0.0", "module": "C2", "scenario": "Standard scenario"}, {"value": "0.0", "module": "C3", "scenario": "Standard scenario"}, {"value": "0.0", "module": "C4", "scenario": "Standard scenario"}, {"value": "0.0", "module": "D", "scenario": "Standard scenario"}, {"name": "referenceToUnitGroupDataSet", "value": {"shortDescription": [{"value": "CTUe", "lang": "en"}], "type": "unit group data set", "refObjectId": "aa959ded-f1eb-4efb-9c5c-2d60be36b3e6", "version": "00.00.003", "uri": "../unitgroups/aa959ded-f1eb-4efb-9c5c-2d60be36b3e6.xml"}}]}}, {"referenceToLCIAMethodDataSet": {"shortDescription": [{"value": "Global Warming Potential - biogenic (GWP-biogenic)", "lang": "en"}, {"value": "Globales Erwärmungspotenzial - biogen (GWP-biogenic)", "lang": "de"}], "type": "LCIA method data set", "refObjectId": "2356e1ab-0185-4db5-86e5-16de51c7485c", "version": "01.00.006", "uri": "../lciamethods/2356e1ab-0185-4db5-86e5-16de51c7485c.xml"}, "meanAmount": 0.0, "other": {"anies": [{"value": "0.0246", "module": "A1", "scenario": "Standard scenario"}, {"value": "2.96E-5", "module": "A2", "scenario": "Standard scenario"}, {"value": "-0.0118", "module": "A3", "scenario": "Standard scenario"}, {"value": "0.0", "module": "C1", "scenario": "Standard scenario"}, {"value": "0.0", "module": "C2", "scenario": "Standard scenario"}, {"value": "0.0", "module": "C3", "scenario": "Standard scenario"}, {"value": "0.0", "module": "C4", "scenario": "Standard scenario"}, {"value": "0.0", "module": "D", "scenario": "Standard scenario"}, {"name": "referenceToUnitGroupDataSet", "value": {"shortDescription": [{"value": "kg CO2-eq.", "lang": "en"}], "type": "unit group data set", "refObjectId": "1ebf3012-d0db-4de2-aefd-ef30cedb0be1", "version": "30.00.000", "uri": "../unitgroups/1ebf3012-d0db-4de2-aefd-ef30cedb0be1.xml"}}]}}, {"referenceToLCIAMethodDataSet": {"shortDescription": [{"value": "Global Warming Potential - fossil fuels (GWP-fossil)", "lang": "en"}, {"value": "Globales Erwärmungspotenzial - fossil (GWP-fossil)", "lang": "de"}], "type": "LCIA method data set", "refObjectId": "5f635281-343e-44fb-83df-1971b155e6b6", "version": "01.00.009", "uri": "../lciamethods/5f635281-343e-44fb-83df-1971b155e6b6.xml"}, "meanAmount": 0.0, "other": {"anies": [{"value": "1.96", "module": "A1", "scenario": "Standard scenario"}, {"value": "0.0642", "module": "A2", "scenario": "Standard scenario"}, {"value": "0.0758", "module": "A3", "scenario": "Standard scenario"}, {"value": "0.0", "module": "C1", "scenario": "Standard scenario"}, {"value": "0.0", "module": "C2", "scenario": "Standard scenario"}, {"value": "0.0", "module": "C3", "scenario": "Standard scenario"}, {"value": "0.0", "module": "C4", "scenario": "Standard scenario"}, {"value": "0.0", "module": "D", "scenario": "Standard scenario"}, {"name": "referenceToUnitGroupDataSet", "value": {"shortDescription": [{"value": "kg CO2-eq.", "lang": "en"}], "type": "unit group data set", "refObjectId": "1ebf3012-d0db-4de2-aefd-ef30cedb0be1", "version": "30.00.000", "uri": "../unitgroups/1ebf3012-d0db-4de2-aefd-ef30cedb0be1.xml"}}]}}, {"referenceToLCIAMethodDataSet": {"shortDescription": [{"value": "Global Warming Potential - land use and land use change (GWP-luluc)", "lang": "en"}, {"value": "Globales Erwärmungspotenzial - luluc (GWP-luluc)", "lang": "de"}], "type": "LCIA method data set", "refObjectId": "4331bbdb-978a-490d-8707-eeb047f01a55", "version": "01.00.006", "uri": "../lciamethods/4331bbdb-978a-490d-8707-eeb047f01a55.xml"}, "meanAmount": 0.0, "other": {"anies": [{"value": "0.00386", "module": "A1", "scenario": "Standard scenario"}, {"value": "2.35E-5", "module": "A2", "scenario": "Standard scenario"}, {"value": "2.82E-4", "module": "A3", "scenario": "Standard scenario"}, {"value": "0.0", "module": "C1", "scenario": "Standard scenario"}, {"value": "0.0", "module": "C2", "scenario": "Standard scenario"}, {"value": "0.0", "module": "C3", "scenario": "Standard scenario"}, {"value": "0.0", "module": "C4", "scenario": "Standard scenario"}, {"value": "0.0", "module": "D", "scenario": "Standard scenario"}, {"name": "referenceToUnitGroupDataSet", "value": {"shortDescription": [{"value": "kg CO2-eq.", "lang": "en"}], "type": "unit group data set", "refObjectId": "1ebf3012-d0db-4de2-aefd-ef30cedb0be1", "version": "30.00.000", "uri": "../unitgroups/1ebf3012-d0db-4de2-aefd-ef30cedb0be1.xml"}}]}}, {"referenceToLCIAMethodDataSet": {"shortDescription": [{"value": "Global Warming Potential - total (GWP-total)", "lang": "en"}, {"value": "Globales Erwärmungspotenzial - total (GWP-total)", "lang": "de"}], "type": "LCIA method data set", "refObjectId": "6a37f984-a4b3-458a-a20a-64418c145fa2", "version": "04.00.017", "uri": "../lciamethods/6a37f984-a4b3-458a-a20a-64418c145fa2.xml"}, "meanAmount": 0.0, "other": {"anies": [{"value": "1.99", "module": "A1", "scenario": "Standard scenario"}, {"value": "0.0642", "module": "A2", "scenario": "Standard scenario"}, {"value": "0.0643", "module": "A3", "scenario": "Standard scenario"}, {"value": "0.0", "module": "C1", "scenario": "Standard scenario"}, {"value": "0.0", "module": "C2", "scenario": "Standard scenario"}, {"value": "0.0", "module": "C3", "scenario": "Standard scenario"}, {"value": "0.0", "module": "C4", "scenario": "Standard scenario"}, {"value": "0.0", "module": "D", "scenario": "Standard scenario"}, {"name": "referenceToUnitGroupDataSet", "value": {"shortDescription": [{"value": "kg CO2-eq.", "lang": "en"}], "type": "unit group data set", "refObjectId": "1ebf3012-d0db-4de2-aefd-ef30cedb0be1", "version": "30.00.000", "uri": "../unitgroups/1ebf3012-d0db-4de2-aefd-ef30cedb0be1.xml"}}]}}, {"referenceToLCIAMethodDataSet": {"shortDescription": [{"value": "Potential Comparative Toxic Unit for humans - cancer effects (HTP-c)", "lang": "en"}, {"value": "Potenzielle Toxizitätsvergleichseinheit für den Menschen - kanzerogene Wirkung (HTP-c)", "lang": "de"}], "type": "LCIA method data set", "refObjectId": "2299222a-bbd8-474f-9d4f-4dd1f18aea7c", "version": "01.00.004", "uri": "../lciamethods/2299222a-bbd8-474f-9d4f-4dd1f18aea7c.xml"}, "meanAmount": 0.0, "other": {"anies": [{"value": "1.55E-8", "module": "A1", "scenario": "Standard scenario"}, {"value": "2.8E-11", "module": "A2", "scenario": "Standard scenario"}, {"value": "3.35E-10", "module": "A3", "scenario": "Standard scenario"}, {"value": "0.0", "module": "C1", "scenario": "Standard scenario"}, {"value": "0.0", "module": "C2", "scenario": "Standard scenario"}, {"value": "0.0", "module": "C3", "scenario": "Standard scenario"}, {"value": "0.0", "module": "C4", "scenario": "Standard scenario"}, {"value": "0.0", "module": "D", "scenario": "Standard scenario"}, {"name": "referenceToUnitGroupDataSet", "value": {"shortDescription": [{"value": "CTUh", "lang": "en"}], "type": "unit group data set", "refObjectId": "d4c9523e-2d7e-49fd-8469-998f547d3a70", "version": "00.00.003", "uri": "../unitgroups/d4c9523e-2d7e-49fd-8469-998f547d3a70.xml"}}]}}, {"referenceToLCIAMethodDataSet": {"shortDescription": [{"value": "Potential Comparative Toxic Unit for humans - non-cancer effects (HTP-nc)", "lang": "en"}, {"value": "Potenzielle Toxizitätsvergleichseinheit für den Menschen - nicht kanzerogene Wirkung (HTP-nc)", "lang": "de"}], "type": "LCIA method data set", "refObjectId": "3af763a5-b7a1-48c9-9cee-1f223481fcef", "version": "01.00.003", "uri": "../lciamethods/3af763a5-b7a1-48c9-9cee-1f223481fcef.xml"}, "meanAmount": 0.0, "other": {"anies": [{"value": "1.11E-7", "module": "A1", "scenario": "Standard scenario"}, {"value": "9.44E-10", "module": "A2", "scenario": "Standard scenario"}, {"value": "2.82E-9", "module": "A3", "scenario": "Standard scenario"}, {"value": "0.0", "module": "C1", "scenario": "Standard scenario"}, {"value": "0.0", "module": "C2", "scenario": "Standard scenario"}, {"value": "0.0", "module": "C3", "scenario": "Standard scenario"}, {"value": "0.0", "module": "C4", "scenario": "Standard scenario"}, {"value": "0.0", "module": "D", "scenario": "Standard scenario"}, {"name": "referenceToUnitGroupDataSet", "value": {"shortDescription": [{"value": "CTUh", "lang": "en"}], "type": "unit group data set", "refObjectId": "d4c9523e-2d7e-49fd-8469-998f547d3a70", "version": "00.00.003", "uri": "../unitgroups/d4c9523e-2d7e-49fd-8469-998f547d3a70.xml"}}]}}, {"referenceToLCIAMethodDataSet": {"shortDescription": [{"value": "Potential Human exposure efficiency relative to U235 (IRP)", "lang": "en"}, {"value": "Potenzielle Wirkung durch Exposition des Menschen mit U235 (IRP)", "lang": "de"}], "type": "LCIA method data set", "refObjectId": "b5c632be-def3-11e6-bf01-fe55135034f3", "version": "01.00.012", "uri": "../lciamethods/b5c632be-def3-11e6-bf01-fe55135034f3.xml"}, "meanAmount": 0.0, "other": {"anies": [{"value": "0.0853", "module": "A1", "scenario": "Standard scenario"}, {"value": "0.00405", "module": "A2", "scenario": "Standard scenario"}, {"value": "0.00423", "module": "A3", "scenario": "Standard scenario"}, {"value": "0.0", "module": "C1", "scenario": "Standard scenario"}, {"value": "0.0", "module": "C2", "scenario": "Standard scenario"}, {"value": "0.0", "module": "C3", "scenario": "Standard scenario"}, {"value": "0.0", "module": "C4", "scenario": "Standard scenario"}, {"value": "0.0", "module": "D", "scenario": "Standard scenario"}, {"name": "referenceToUnitGroupDataSet", "value": {"shortDescription": [{"value": "kgBq U235-eq.", "lang": "en"}], "type": "unit group data set", "refObjectId": "456b05bf-1415-44a9-9993-02452f554c09", "version": "00.00.003", "uri": "../unitgroups/456b05bf-1415-44a9-9993-02452f554c09.xml"}}]}}, {"referenceToLCIAMethodDataSet": {"shortDescription": [{"value": "Depletion potential of the stratospheric ozone layer (ODP)", "lang": "en"}, {"value": "Abbaupotenzial der stratosphärischen Ozonschicht (ODP)", "lang": "de"}], "type": "LCIA method data set", "refObjectId": "b5c629d6-def3-11e6-bf01-fe55135034f3", "version": "02.00.013", "uri": "../lciamethods/b5c629d6-def3-11e6-bf01-fe55135034f3.xml"}, "meanAmount": 0.0, "other": {"anies": [{"value": "4.56E-7", "module": "A1", "scenario": "Standard scenario"}, {"value": "1.42E-8", "module": "A2", "scenario": "Standard scenario"}, {"value": "1.3E-8", "module": "A3", "scenario": "Standard scenario"}, {"value": "0.0", "module": "C1", "scenario": "Standard scenario"}, {"value": "0.0", "module": "C2", "scenario": "Standard scenario"}, {"value": "0.0", "module": "C3", "scenario": "Standard scenario"}, {"value": "0.0", "module": "C4", "scenario": "Standard scenario"}, {"value": "0.0", "module": "D", "scenario": "Standard scenario"}, {"name": "referenceToUnitGroupDataSet", "value": {"shortDescription": [{"value": "kg CFC-11-eq.", "lang": "en"}], "type": "unit group data set", "refObjectId": "d9e957c9-7309-4474-bf3a-7777df6c4e5b", "version": "25.00.000", "uri": "../unitgroups/d9e957c9-7309-4474-bf3a-7777df6c4e5b.xml"}}]}}, {"referenceToLCIAMethodDataSet": {"shortDescription": [{"value": "Potential incidence of disease due to PM emissions (PM)", "lang": "en"}, {"value": "Potenzielles Auftreten von Krankheiten aufgrund von Feinstaubemissionen (PM)", "lang": "de"}], "type": "LCIA method data set", "refObjectId": "b5c602c6-def3-11e6-bf01-fe55135034f3", "version": "02.00.012", "uri": "../lciamethods/b5c602c6-def3-11e6-bf01-fe55135034f3.xml"}, "meanAmount": 0.0, "other": {"anies": [{"value": "6.44E-8", "module": "A1", "scenario": "Standard scenario"}, {"value": "5.77E-9", "module": "A2", "scenario": "Standard scenario"}, {"value": "6.94E-9", "module": "A3", "scenario": "Standard scenario"}, {"value": "0.0", "module": "C1", "scenario": "Standard scenario"}, {"value": "0.0", "module": "C2", "scenario": "Standard scenario"}, {"value": "0.0", "module": "C3", "scenario": "Standard scenario"}, {"value": "0.0", "module": "C4", "scenario": "Standard scenario"}, {"value": "0.0", "module": "D", "scenario": "Standard scenario"}, {"name": "referenceToUnitGroupDataSet", "value": {"shortDescription": [{"value": "Disease incidence", "lang": "en"}], "type": "unit group data set", "refObjectId": "3883559b-648f-4afc-8ba2-0bd24f3affa3", "version": "00.00.003", "uri": "../unitgroups/3883559b-648f-4afc-8ba2-0bd24f3affa3.xml"}}]}}, {"referenceToLCIAMethodDataSet": {"shortDescription": [{"value": "Photochemical Ozone Creation Potential (POCP)", "lang": "en"}, {"value": "Bildungspotenzial für troposphärisches Ozon (POCP)", "lang": "de"}], "type": "LCIA method data set", "refObjectId": "b5c610fe-def3-11e6-bf01-fe55135034f3", "version": "02.00.015", "uri": "../lciamethods/b5c610fe-def3-11e6-bf01-fe55135034f3.xml"}, "meanAmount": 0.0, "other": {"anies": [{"value": "0.00712", "module": "A1", "scenario": "Standard scenario"}, {"value": "4.13E-4", "module": "A2", "scenario": "Standard scenario"}, {"value": "2.99E-4", "module": "A3", "scenario": "Standard scenario"}, {"value": "0.0", "module": "C1", "scenario": "Standard scenario"}, {"value": "0.0", "module": "C2", "scenario": "Standard scenario"}, {"value": "0.0", "module": "C3", "scenario": "Standard scenario"}, {"value": "0.0", "module": "C4", "scenario": "Standard scenario"}, {"value": "0.0", "module": "D", "scenario": "Standard scenario"}, {"name": "referenceToUnitGroupDataSet", "value": {"shortDescription": [{"value": "kg NMVOC-eq.", "lang": "en"}], "type": "unit group data set", "refObjectId": "d27c25f8-fbc1-44c6-b47b-4adbae4199c6", "version": "00.00.003", "uri": "../unitgroups/d27c25f8-fbc1-44c6-b47b-4adbae4199c6.xml"}}]}}, {"referenceToLCIAMethodDataSet": {"shortDescription": [{"value": "Potential Soil quality index (SQP)", "lang": "en"}, {"value": "Potenzieller Bodenqualitätsindex (SQP)", "lang": "de"}], "type": "LCIA method data set", "refObjectId": "b2ad6890-c78d-11e6-9d9d-cec0c932ce01", "version": "01.00.011", "uri": "../lciamethods/b2ad6890-c78d-11e6-9d9d-cec0c932ce01.xml"}, "meanAmount": 0.0, "other": {"anies": [{"value": "205.0", "module": "A1", "scenario": "Standard scenario"}, {"value": "0.839", "module": "A2", "scenario": "Standard scenario"}, {"value": "8.9", "module": "A3", "scenario": "Standard scenario"}, {"value": "0.0", "module": "C1", "scenario": "Standard scenario"}, {"value": "0.0", "module": "C2", "scenario": "Standard scenario"}, {"value": "0.0", "module": "C3", "scenario": "Standard scenario"}, {"value": "0.0", "module": "C4", "scenario": "Standard scenario"}, {"value": "0.0", "module": "D", "scenario": "Standard scenario"}, {"name": "referenceToUnitGroupDataSet", "value": {"shortDescription": [{"value": "dimensionless", "lang": "en"}], "type": "unit group data set", "refObjectId": "f130951c-e67f-4f7f-8dd4-665de3974e18", "version": "00.00.004", "uri": "../unitgroups/f130951c-e67f-4f7f-8dd4-665de3974e18.xml"}}]}}, {"referenceToLCIAMethodDataSet": {"shortDescription": [{"value": "Water (user) deprivation potential (WDP)", "lang": "en"}, {"value": "Wasser-Entzugspotenzial (Benutzer) (WDP)", "lang": "de"}], "type": "LCIA method data set", "refObjectId": "b2ad66ce-c78d-11e6-9d9d-cec0c932ce01", "version": "03.00.015", "uri": "../lciamethods/b2ad66ce-c78d-11e6-9d9d-cec0c932ce01.xml"}, "meanAmount": 0.0, "other": {"anies": [{"value": "0.0294", "module": "A1", "scenario": "Standard scenario"}, {"value": "0.00346", "module": "A2", "scenario": "Standard scenario"}, {"value": "0.0121", "module": "A3", "scenario": "Standard scenario"}, {"value": "0.0", "module": "C1", "scenario": "Standard scenario"}, {"value": "0.0", "module": "C2", "scenario": "Standard scenario"}, {"value": "0.0", "module": "C3", "scenario": "Standard scenario"}, {"value": "0.0", "module": "C4", "scenario": "Standard scenario"}, {"value": "0.0", "module": "D", "scenario": "Standard scenario"}, {"name": "referenceToUnitGroupDataSet", "value": {"shortDescription": [{"value": "m3 world eq. deprived", "lang": "en"}], "type": "unit group data set", "refObjectId": "6ae2df01-888e-46c8-b17d-49fa3869b476", "version": "00.00.003", "uri": "../unitgroups/6ae2df01-888e-46c8-b17d-49fa3869b476.xml"}}]}}]}, "otherAttributes": {"{http://www.indata.network/EPD/2019}epd-version": "1.2"}, "version": "1.1"}