{"processInformation": {"dataSetInformation": {"UUID": "ef9fb0ef-36d3-480b-a8fe-83379dd36bbf", "name": {"baseName": [{"value": "noraplan® ultra grip", "lang": "de"}, {"value": "noraplan® ultra grip", "lang": "en"}], "functionalUnitFlowProperties": [{"lang": "de"}]}, "classificationInformation": {"classification": [{"class": [{"value": "Kunststoffe", "level": 0, "classId": "6"}, {"value": "Bodenbeläge", "level": 1, "classId": "6.2"}, {"value": "Gummi-/Kautschuk-Bodenbeläge", "level": 2, "classId": "6.2.02"}], "name": "OEKOBAU.DAT"}, {"class": [{"value": "02 Bauprodukte", "level": 0}, {"value": "Bodenbeläge", "level": 1}, {"value": "Bodenbeläge", "level": 2}], "name": "IBUCategories"}]}, "generalComment": [{"value": "In dieser Umwelt-Produktdeklaration (EDP) werden elastische Kautschuk-Sicherheitsbodenbeläge für erhöhte Rutschsicherheit der nora systems GmbH der Produktfamilie noraplan® ultra grip abgebildet.", "lang": "de"}, {"value": "In this Environmental Product Declaration (EPD), resilient rubber floor coverings with a high slip resistance of the nora systems GmbH product line noraplan® ultra grip are modelled. \n\nFor the product line noraplan® ultra grip standards apply:\n\nEN 1817:2007-7: Resilient floor coverings - Specification for homogeneous and heterogeneous smooth rubber floor coverings\nEN 14521:2004-9: Resilient floor coverings -Specification for smooth rubber floor coverings with or without foam backing with a decorative layer\nISO 10874:2009-11: Resilient, textile and laminate floor coverings – Classification", "lang": "en"}]}, "quantitativeReference": {"referenceToReferenceFlow": [0]}, "time": {"referenceYear": 2022, "dataSetValidUntil": 2027, "other": {"anies": [{"name": "publicationDateOfEPD", "value": 1644883200000}]}}, "geography": {"locationOfOperationSupplyOrProduction": {"location": "RER"}}, "technology": {"technologyDescriptionAndIncludedProcesses": [{"value": "Die Produktionsstufen sind Einwiegen, Mischen und Ausziehen der unvulkanisierten Rohlinge auf einem Kalander. Die anschließende Vulkanisation erfolgt kontinuierlich auf Fertigungslinien mit dampfbeheizten Trommelpressen unter hohem Druck bei einer Temperatur von ca. 180°C zu 1,22 m breiten Bahnen. Hinter der Vulkanisationsmaschine werden die Bahnen rückseitig geschliffen und als Rollenware aufgewickelt. Das Flächengewicht beträgt 3,36 kg/m². Das Qualitätsmanagement der nora Systems GmbH ist nach ISO 9001 zertifiziert. \nTechnische Daten: \nAuszug aus technischen Datenblättern: (abrufbar auf www.nora.com) \nDeklarierte Einheit: \nAls Referenzgröße wird 1 m² Bodenbelag betrachtet. Die Werte des Moduls A1- A3 beziehen sich auf 1 m² produziertes Produkt.\n\nEs handelt sich um eine Produktdeklaration. Die Herstellung und Beseitigung der Verschnitte bei der Installation werden dem Modul A5 zugeordnet. Die Module A1- A3, A4 und A5 beziehen sich gesamt auf\n\n1 m² installiertes Produkt.\n\nDie zur Installation notwendigen Materialien zur Vorbereitung des Untergrunds und zur Klebung werden nicht berücksichtigt. Für den vollständigen Bodenaufbau können Umweltproduktdeklarationen nach den PCR „Dispersionsklebstoffe und – voranstriche“ sowie „Mineralische Werkmörtel“ herangezogen werden.", "lang": "de"}, {"value": "The production stages are weighing, mixing, and stretching of the unvulcanized blanks on a calender. The following vulcanization is continuously executed on production lines with steam heated drum presses, where under high pressure and at a temperature of approximately 180°C sheets of 1.22 m width are produced. After the vulcanization machine, the sheets are backside sanded and either wound into rolls or, for tiles, cut to length and die-cut. The mass per unit area is 3,36 kg/m². The quality and energy management of nora systems GmbH is certified according to ISO 9001. \nTechnical data: \nExcerpt of technical data sheets: (available at www.nora.com) \nDeclared unit: \nThe reference unit is 1 m² of floor covering. The values of module A1- A3 refer to 1 m² produced. This EPD represents a product declaration, i.e. the production and disposal of off-cuts during installation the stage are assigned to module A5. The combined modules A1- A3, A4 and A5 refer to a reference unit of 1 m² installed.\n\n\nThe material for subfloor preparation and adhesive bonding, needed during installation, is not considered. Information on the complete floor structure can be found in Environmental Product Declarations based on the PCR „Dispersion adhesives and primers for floor coverings“ and „Mineral factory-made mortar”.", "lang": "en"}], "technologicalApplicability": [{"value": "noraplan® ultra grip Bodenbeläge bieten eine erhöhte Rutschsicherheit, R11 nach DIN 51130 und 36+ im TRRL Pendulum Test. Zudem sind die noraplan® ultra grip Bodenbeläge weitgehend beständig gegen viele Öle und Schmierfette. Die Bodenbeläge werden gemäß ISO 10874 klassifiziert.\n\nBodenbeläge für starke Beanspruchung im Privat- und\n\n Objektbereich:", "lang": "de"}, {"value": "Electrostatically dissipative noraplan® ultra grip floorings offer optimum ESD protection of electronic devices and equipment. It protects against electrical shock and is resisting most oils and greases.\n\nFloor coverings are classified according to ISO 10874. \n\nFloor coverings for high performance  in professional use:", "lang": "en"}]}}, "modellingAndValidation": {"LCIMethodAndAllocation": {"typeOfDataSet": "EPD", "referenceToLCAMethodDetails": [{"shortDescription": [{"value": "Bodenbeläge.pdf", "lang": "de"}], "type": "source data set", "refObjectId": "c2067768-3a36-47f7-b729-4b8f2918e069"}], "other": {"anies": [{"name": "subType", "value": "specific dataset"}]}}, "dataSourcesTreatmentAndRepresentativeness": {"referenceToDataSource": [{"shortDescription": [{"value": "GaBi Database (all versions)", "lang": "de"}], "type": "source data set", "refObjectId": "28d74cc0-db8b-4d7e-bc44-5f6d56ce0c4a"}, {"shortDescription": [{"value": "GaBi Database Edition 2021, CUP 2021.01", "lang": "de"}], "type": "source data set", "refObjectId": "1cece811-7501-44d4-8067-9259bd5cb835"}], "useAdviceForDataSet": [{"value": "Gültigkeitsbereich: \nProduktfamilie noraplan® ultra grip. Kontinuierlich in Bahnen vulkanisierte Sicherheitsbodenbeläge aus Kautschuk in verschiedenen Farben und Designs. Diese Deklaration ist eine Umweltproduktdeklaration gemäß ISO 14025 und EN 15804 und beschreibt die spezifische Umweltleistung der hier genannten Bauprodukte, produziert in Deutschland am Produktionsstandort Weinheim (Bergstraße). \nSystemgrenze: \nTyp der EPD: von der Wiege bis zum Fabriktor mit\n\nOptionen.\n\nDie ökobilanzielle Berechnung umfasst folgende\n\nPhasen:\n\nHerstellungsphase A1- A3: Berücksichtigung der Vorkette und der Produktion des Bodenbelags, inkl. Verpackung (Input von Altpapier bei der Papier-/Kartonherstellung).\nTransport A4: Annahme für den Transport der Produkte zur Baustelle.\nInstallationsphase A5: Berücksichtigung der Herstellung und des Transports der Verschnittmenge, Verbrennung des Verschnitts (gewonnene Energie wird in D als vermiedene Umweltlasten deklariert), Entsorgung der Verpackungsmaterialien (Verbrennung von Polyethylenfolie). Die Untergrundvorbehandlung (Grundierung, Spachtelmasse, Klebstoff) bleibt unberücksichtigt. Diese ist abhängig vom Gebäude und der Anwendung und muss im Einzelfall spezifiziert werden.\nNutzungsphase B2: Szenario für die Reinigung entsprechend den Herstellerempfehlungen (siehe 4.).\n End-of-Life-Phase C1, C2, C3: Szenario für die Verbrennung des Bodenbelags inkl. Ausbau aus dem Gebäude und Transport zum Verbrennungsort (gewonnene Energie wird in D als vermiedene Umweltlasten deklariert).\nNutzen und Lasten für das nächste System D: Gewinnung von elektrischer und thermischer Energie aus der thermischen Verwertung des Produkts, des Installationsverschnitts und der VerpackungEinflüsse von Abfällen werden in den Modulen berücksichtigt, in denen diese anfallen.", "lang": "de"}, {"value": "Scope: \nProduct line noraplan® ultra grip \n\nSafety rubber floor coverings continuously vulcanized in sheets in various colors and designs.\n\nThis declaration is an Environmental Product Declaration according to ISO 14025 and EN 15804 describing the specific environmental performance of the mentioned construction products produced in Germany (Weinheim/Bergstraße). \nSystem boundary: \nType of EPD: from cradle to gate with options\n\nThe analysis of the product life cycle includes the\n\nfollowing stages:\n\nProduction stage A1- A3: Consideration of production of the basic materials and the manufacturing of the floor covering incl. packaging material (input of waste paper for paper/cardboard production).\nTransport A4: Assumption for the transport of the products to the construction site.\nInstallation A5: Production, transport and incineration of the off-cut material, incineration of off-cut material (gained energy is declared in D as avoided environmental burden), disposal of the packaging (incineration of PE film). The pretreatment of the underground surface (prime coat, levelling compound, adhesive) is not considered. This treatment depends on the building and the application and need to be specified for the particular case.\nUse stage B2: Scenario for maintenance/cleaning according to the manufacturer's recommendation (see 4.)\nEnd-of-Life stage C1, C2, C3: Scenario for the incineration of the floor covering incl. removal from the building and transport to the waste incineration plant (gained energy is declared in D as avoided environmental burden).\nBenefits for the next product system D: Extraction for electrical and thermal energy from the waste incineration process of the product, the off-cuts and the packaging material.\n\nContributions of waste flows are considered in the modules where they occur.", "lang": "en"}], "other": {"anies": [{"name": "referenceToOriginalEPD", "value": {"shortDescription": {"value": "noraplan® ultra grip.pdf", "defaultValue": "noraplan® ultra grip.pdf", "lstrings": [{"lang": "de", "value": "noraplan® ultra grip.pdf"}]}, "type": "source data set", "uuid": {"uuid": "53f9d069-3061-4cdf-9ea6-a94ceb44a14a"}, "refObjectId": "53f9d069-3061-4cdf-9ea6-a94ceb44a14a", "resourceURLs": ["https://oekobaudat.de/OEKOBAU.DAT/resource/sources/53f9d069-3061-4cdf-9ea6-a94ceb44a14a/noraplan_ultra_grip_15334.pdf?version=00.01.000"]}}]}}, "validation": {"review": [{"referenceToNameOfReviewerAndInstitution": [{"shortDescription": [{"value": "Institut Bauen und Umwelt e. V.", "lang": "de"}], "type": "contact data set", "refObjectId": "d111dbec-b024-4be5-86c5-752d6eb2cf95", "uri": "../contacts/d111dbec-b024-4be5-86c5-752d6eb2cf95.xml"}], "type": "Accredited third party review"}]}, "complianceDeclarations": {"compliance": [{"referenceToComplianceSystem": {"shortDescription": [{"value": "DIN EN 15804+A2", "lang": "de"}], "type": "source data set", "refObjectId": "c0016b33-8cf7-415c-ac6e-deba0d21440d", "uri": "../sources/c0016b33-8cf7-415c-ac6e-deba0d21440d.xml"}}, {"referenceToComplianceSystem": {"shortDescription": [{"value": "ISO 14025", "lang": "de"}], "type": "source data set", "refObjectId": "4f2eb655-6e44-4874-a95a-e28f5442cd4d", "uri": "../sources/4f2eb655-6e44-4874-a95a-e28f5442cd4d.xml"}}]}}, "administrativeInformation": {"commissionerAndGoal": {"referenceToCommissioner": [{"shortDescription": [{"value": "nora systems GmbH", "lang": "de"}], "type": "contact data set", "refObjectId": "6116f444-2f51-49a2-8f7e-82c2cbb7f3ff", "uri": "../contacts/6116f444-2f51-49a2-8f7e-82c2cbb7f3ff.xml"}]}, "dataGenerator": {"referenceToPersonOrEntityGeneratingTheDataSet": [{"shortDescription": [{"value": "nora systems GmbH", "lang": "de"}], "type": "contact data set", "refObjectId": "6116f444-2f51-49a2-8f7e-82c2cbb7f3ff", "uri": "../contacts/6116f444-2f51-49a2-8f7e-82c2cbb7f3ff.xml"}]}, "dataEntryBy": {"timeStamp": 1644918282267, "referenceToDataSetFormat": [{"shortDescription": [{"value": "ILCD Format", "lang": "de"}], "type": "source data set", "refObjectId": "a97a0155-0234-4b87-b4ce-a45da52f2a40", "uri": "../sources/a97a0155-0234-4b87-b4ce-a45da52f2a40.xml"}, {"shortDescription": [{"value": "EPD-Datenformaterweiterungen v1.2", "lang": "de"}, {"value": "EPD Data Format Extensions v1.2", "lang": "en"}], "type": "source data set", "refObjectId": "a29449fd-aa2f-4de8-b5d7-4b06b43c6fde", "uri": "../sources/a29449fd-aa2f-4de8-b5d7-4b06b43c6fde.xml"}]}, "publicationAndOwnership": {"dataSetVersion": "00.01.000", "referenceToRegistrationAuthority": {"shortDescription": [{"value": "Institut Bauen und Umwelt e. V.", "lang": "de"}], "type": "contact data set", "refObjectId": "d111dbec-b024-4be5-86c5-752d6eb2cf95", "uri": "../contacts/d111dbec-b024-4be5-86c5-752d6eb2cf95.xml"}, "registrationNumber": "EPD-NOR-2022005-IBA1-DE", "referenceToOwnershipOfDataSet": {"shortDescription": [{"value": "nora systems GmbH", "lang": "de"}], "type": "contact data set", "refObjectId": "6116f444-2f51-49a2-8f7e-82c2cbb7f3ff", "uri": "../contacts/6116f444-2f51-49a2-8f7e-82c2cbb7f3ff.xml"}, "copyright": true, "licenseType": "Free of charge for all users and uses", "accessRestrictions": [{"value": "None", "lang": "en"}], "other": {"anies": [{"name": "referenceToPublisher", "value": {"shortDescription": [{"value": "Institut Bauen und Umwelt e. V.", "lang": "de"}], "type": "contact data set", "refObjectId": "d111dbec-b024-4be5-86c5-752d6eb2cf95", "uri": "../contacts/d111dbec-b024-4be5-86c5-752d6eb2cf95.xml"}}]}}}, "exchanges": {"exchange": [{"dataSetInternalID": 0, "referenceToFlowDataSet": {"shortDescription": [{"value": "noraplan ultra grip ()", "lang": "de"}], "type": "flow data set", "refObjectId": "f499cd4c-1e79-2ac6-5b59-b0012e789a40", "uri": "../flows/f499cd4c-1e79-2ac6-5b59-b0012e789a40.xml"}, "meanAmount": 1.0, "referencesToDataSource": {}, "referenceFlow": true, "resolvedFlowVersion": "00.01.000", "resultingflowAmount": 1.0, "flowProperties": [{"name": [{"lang": "en", "value": "Area"}, {"lang": "de", "value": "Fläche"}], "uuid": "93a60a56-a3c8-19da-a746-0800200c9a66", "referenceFlowProperty": true, "meanValue": 1.0, "referenceUnit": "qm", "unitGroupUUID": "c20a03d7-bd90-4569-bc94-66cfd364dfc8"}], "materialProperties": [{"name": "layer thickness", "value": "2.0", "unit": "m", "unitDescription": "meters"}, {"name": "layer thickness", "value": "0.002", "unit": "m", "unitDescription": "meters"}, {"name": "conversion factor [mass/declared unit]", "value": "3.36", "unit": "-", "unitDescription": "Without unit"}, {"name": "grammage", "value": "3.36", "unit": "kg/m^2", "unitDescription": "kilograms per square meter"}, {"name": "gross density", "value": "3.36", "unit": "kg/m^3", "unitDescription": "kilograms per cubic metre"}], "typeOfFlow": "Product flow", "classification": {"classHierarchy": "Kunststoffe / Bodenbeläge / Gummi-/Kautschuk-Bodenbeläge", "name": "OEKOBAU.DAT"}}, {"dataSetInternalID": 1, "referenceToFlowDataSet": {"shortDescription": [{"value": "Erneuerbare Primärenergie als Energieträger (PERE)", "lang": "de"}, {"value": "Renewable primary energy as energy carrier (PERE)", "lang": "en"}], "type": "flow data set", "refObjectId": "20f32be5-0398-4288-9b6d-accddd195317", "uri": "../flows/20f32be5-0398-4288-9b6d-accddd195317.xml"}, "exchange direction": "INPUT", "other": {"anies": [{"name": "referenceToUnitGroupDataSet", "value": {"shortDescription": [{"value": "MJ", "lang": "de"}], "type": "unit group data set", "refObjectId": "93a60a57-a3c8-11da-a746-0800200c9a66", "uri": "../unitgroups/93a60a57-a3c8-11da-a746-0800200c9a66.xml"}}, {"value": "20.8085208384359", "module": "A1-A3"}, {"value": "0.124262775472858", "module": "A4"}, {"value": "2.77465795119439", "module": "A5"}, {"value": "0.456396634933545", "module": "B2"}, {"value": "0.325931103033835", "module": "C1"}, {"value": "0.00616531081174225", "module": "C2"}, {"value": "1.14673433709701", "module": "C3"}, {"value": "-4.4430690011035", "module": "D"}]}, "resolvedFlowVersion": "38.00.000", "flowProperties": [], "typeOfFlow": "Other flow", "classification": {"classHierarchy": "Quantities", "name": "GaBiCategories"}}, {"dataSetInternalID": 2, "referenceToFlowDataSet": {"shortDescription": [{"value": "Erneuerbare Primärenergie zur stofflichen Nutzung (PERM)", "lang": "de"}, {"value": "Renewable primary energy resources as material utilization (PERM)", "lang": "en"}], "type": "flow data set", "refObjectId": "fb3ec0de-548d-4508-aea5-00b73bf6f702", "uri": "../flows/fb3ec0de-548d-4508-aea5-00b73bf6f702.xml"}, "exchange direction": "INPUT", "other": {"anies": [{"name": "referenceToUnitGroupDataSet", "value": {"shortDescription": [{"value": "MJ", "lang": "de"}], "type": "unit group data set", "refObjectId": "93a60a57-a3c8-11da-a746-0800200c9a66", "uri": "../unitgroups/93a60a57-a3c8-11da-a746-0800200c9a66.xml"}}, {"value": "2.60329464285714", "module": "A1-A3"}, {"value": "0", "module": "A4"}, {"value": "-1.55329464285714", "module": "A5"}, {"value": "0", "module": "B2"}, {"value": "0", "module": "C1"}, {"value": "0", "module": "C2"}, {"value": "-1.05", "module": "C3"}, {"value": "0", "module": "D"}]}, "resolvedFlowVersion": "38.00.000", "flowProperties": [], "typeOfFlow": "Other flow", "classification": {"classHierarchy": "Quantities", "name": "GaBiCategories"}}, {"dataSetInternalID": 3, "referenceToFlowDataSet": {"shortDescription": [{"value": "Total erneuerbare Primärenergie (PERT)", "lang": "de"}, {"value": "Total use of renewable primary energy resources (PERT)", "lang": "en"}], "type": "flow data set", "refObjectId": "53f97275-fa8a-4cdd-9024-65936002acd0", "uri": "../flows/53f97275-fa8a-4cdd-9024-65936002acd0.xml"}, "exchange direction": "INPUT", "other": {"anies": [{"name": "referenceToUnitGroupDataSet", "value": {"shortDescription": [{"value": "MJ", "lang": "de"}], "type": "unit group data set", "refObjectId": "93a60a57-a3c8-11da-a746-0800200c9a66", "uri": "../unitgroups/93a60a57-a3c8-11da-a746-0800200c9a66.xml"}}, {"value": "23.411815481293", "module": "A1-A3"}, {"value": "0.124262775472858", "module": "A4"}, {"value": "1.22136330833725", "module": "A5"}, {"value": "0.456396634933545", "module": "B2"}, {"value": "0.325931103033835", "module": "C1"}, {"value": "0.00616531081174225", "module": "C2"}, {"value": "0.0967343370970084", "module": "C3"}, {"value": "-4.4430690011035", "module": "D"}]}, "resolvedFlowVersion": "38.00.000", "flowProperties": [], "typeOfFlow": "Other flow", "classification": {"classHierarchy": "Quantities / Environmental quantities / EPD EN 15804 / LCI indicators", "name": "GaBiCategories"}}, {"dataSetInternalID": 4, "referenceToFlowDataSet": {"shortDescription": [{"value": "Nicht-erneuerbare Primärenergie als Energieträger (PENRE)", "lang": "de"}, {"value": "Non renewable primary energy as energy carrier (PENRE)", "lang": "en"}], "type": "flow data set", "refObjectId": "ac857178-2b45-46ec-892a-a9a4332f0372", "uri": "../flows/ac857178-2b45-46ec-892a-a9a4332f0372.xml"}, "exchange direction": "INPUT", "other": {"anies": [{"name": "referenceToUnitGroupDataSet", "value": {"shortDescription": [{"value": "MJ", "lang": "de"}], "type": "unit group data set", "refObjectId": "93a60a57-a3c8-11da-a746-0800200c9a66", "uri": "../unitgroups/93a60a57-a3c8-11da-a746-0800200c9a66.xml"}}, {"value": "146.924927582863", "module": "A1-A3"}, {"value": "2.42714316865937", "module": "A4"}, {"value": "10.3507202914991", "module": "A5"}, {"value": "8.05376562684174", "module": "B2"}, {"value": "0.707349624048039", "module": "C1"}, {"value": "0.107533787067371", "module": "C2"}, {"value": "48.3357852614414", "module": "C3"}, {"value": "-19.5484731142934", "module": "D"}]}, "resolvedFlowVersion": "38.00.000", "flowProperties": [], "typeOfFlow": "Other flow", "classification": {"classHierarchy": "Quantities", "name": "GaBiCategories"}}, {"dataSetInternalID": 5, "referenceToFlowDataSet": {"shortDescription": [{"value": "Nicht-erneuerbare Primärenergie zur stofflichen Nutzung (PENRM)", "lang": "de"}, {"value": "Non renewable primary energy as material utilization (PENRM)", "lang": "en"}], "type": "flow data set", "refObjectId": "1421caa0-679d-4bf4-b282-0eb850ccae27", "uri": "../flows/1421caa0-679d-4bf4-b282-0eb850ccae27.xml"}, "exchange direction": "INPUT", "other": {"anies": [{"name": "referenceToUnitGroupDataSet", "value": {"shortDescription": [{"value": "MJ", "lang": "de"}], "type": "unit group data set", "refObjectId": "93a60a57-a3c8-11da-a746-0800200c9a66", "uri": "../unitgroups/93a60a57-a3c8-11da-a746-0800200c9a66.xml"}}, {"value": "47.9799", "module": "A1-A3"}, {"value": "0", "module": "A4"}, {"value": "-0.1299", "module": "A5"}, {"value": "0", "module": "B2"}, {"value": "0", "module": "C1"}, {"value": "0", "module": "C2"}, {"value": "-47.85", "module": "C3"}, {"value": "0", "module": "D"}]}, "resolvedFlowVersion": "38.00.000", "flowProperties": [], "typeOfFlow": "Other flow", "classification": {"classHierarchy": "Quantities", "name": "GaBiCategories"}}, {"dataSetInternalID": 6, "referenceToFlowDataSet": {"shortDescription": [{"value": "Total nicht erneuerbare Primärenergie (PENRT)", "lang": "de"}, {"value": "Total use of non renewable primary energy resources (PENRT)", "lang": "en"}], "type": "flow data set", "refObjectId": "06159210-646b-4c8d-8583-da9b3b95a6c1", "uri": "../flows/06159210-646b-4c8d-8583-da9b3b95a6c1.xml"}, "exchange direction": "INPUT", "other": {"anies": [{"name": "referenceToUnitGroupDataSet", "value": {"shortDescription": [{"value": "MJ", "lang": "de"}], "type": "unit group data set", "refObjectId": "93a60a57-a3c8-11da-a746-0800200c9a66", "uri": "../unitgroups/93a60a57-a3c8-11da-a746-0800200c9a66.xml"}}, {"value": "194.904827582863", "module": "A1-A3"}, {"value": "2.42714316865937", "module": "A4"}, {"value": "10.2208202914991", "module": "A5"}, {"value": "8.05376562684174", "module": "B2"}, {"value": "0.707349624048039", "module": "C1"}, {"value": "0.107533787067371", "module": "C2"}, {"value": "0.485785261441365", "module": "C3"}, {"value": "-19.5484731142934", "module": "D"}]}, "resolvedFlowVersion": "38.00.000", "flowProperties": [], "typeOfFlow": "Other flow", "classification": {"classHierarchy": "Quantities / Environmental quantities / EPD EN 15804 / LCI indicators", "name": "GaBiCategories"}}, {"dataSetInternalID": 7, "referenceToFlowDataSet": {"shortDescription": [{"value": "Einsatz von Sekundärstoffen (SM)", "lang": "de"}, {"value": "Use of secondary material (SM)", "lang": "en"}], "type": "flow data set", "refObjectId": "c6a1f35f-2d09-4f54-8dfb-97e502e1ce92", "uri": "../flows/c6a1f35f-2d09-4f54-8dfb-97e502e1ce92.xml"}, "exchange direction": "INPUT", "other": {"anies": [{"name": "referenceToUnitGroupDataSet", "value": {"shortDescription": [{"value": "kg", "lang": "de"}], "type": "unit group data set", "refObjectId": "ad38d542-3fe9-439d-9b95-2f5f7752acaf", "uri": "../unitgroups/ad38d542-3fe9-439d-9b95-2f5f7752acaf.xml"}}, {"value": "0.170280717938302", "module": "A1-A3"}, {"value": "0", "module": "A4"}, {"value": "0.0085140358969151", "module": "A5"}, {"value": "0", "module": "B2"}, {"value": "0", "module": "C1"}, {"value": "0", "module": "C2"}, {"value": "0", "module": "C3"}, {"value": "0", "module": "D"}]}, "resolvedFlowVersion": "38.00.000", "flowProperties": [], "typeOfFlow": "Other flow", "classification": {"classHierarchy": "Quantities / Environmental quantities / EPD EN 15804 / LCI indicators", "name": "GaBiCategories"}}, {"dataSetInternalID": 8, "referenceToFlowDataSet": {"shortDescription": [{"value": "Erneuerbare Sekundärbrennstoffe (RSF)", "lang": "de"}, {"value": "Use of renewable secondary fuels (RSF)", "lang": "en"}], "type": "flow data set", "refObjectId": "64333088-a55f-4aa2-9a31-c10b07816787", "uri": "../flows/64333088-a55f-4aa2-9a31-c10b07816787.xml"}, "exchange direction": "INPUT", "other": {"anies": [{"name": "referenceToUnitGroupDataSet", "value": {"shortDescription": [{"value": "MJ", "lang": "de"}], "type": "unit group data set", "refObjectId": "93a60a57-a3c8-11da-a746-0800200c9a66", "uri": "../unitgroups/93a60a57-a3c8-11da-a746-0800200c9a66.xml"}}, {"value": "0", "module": "A1-A3"}, {"value": "0", "module": "A4"}, {"value": "0", "module": "A5"}, {"value": "0", "module": "B2"}, {"value": "0", "module": "C1"}, {"value": "0", "module": "C2"}, {"value": "0", "module": "C3"}, {"value": "0", "module": "D"}]}, "resolvedFlowVersion": "38.00.000", "flowProperties": [], "typeOfFlow": "Other flow", "classification": {"classHierarchy": "Quantities / Environmental quantities / EPD EN 15804 / LCI indicators", "name": "GaBiCategories"}}, {"dataSetInternalID": 9, "referenceToFlowDataSet": {"shortDescription": [{"value": "Nicht erneuerbare Sekundärbrennstoffe (NRSF)", "lang": "de"}, {"value": "Use of non renewable secondary fuels (NRSF)", "lang": "en"}], "type": "flow data set", "refObjectId": "89def144-d39a-4287-b86f-efde453ddcb2", "uri": "../flows/89def144-d39a-4287-b86f-efde453ddcb2.xml"}, "exchange direction": "INPUT", "other": {"anies": [{"name": "referenceToUnitGroupDataSet", "value": {"shortDescription": [{"value": "MJ", "lang": "de"}], "type": "unit group data set", "refObjectId": "93a60a57-a3c8-11da-a746-0800200c9a66", "uri": "../unitgroups/93a60a57-a3c8-11da-a746-0800200c9a66.xml"}}, {"value": "0", "module": "A1-A3"}, {"value": "0", "module": "A4"}, {"value": "0", "module": "A5"}, {"value": "0", "module": "B2"}, {"value": "0", "module": "C1"}, {"value": "0", "module": "C2"}, {"value": "0", "module": "C3"}, {"value": "0", "module": "D"}]}, "resolvedFlowVersion": "38.00.000", "flowProperties": [], "typeOfFlow": "Other flow", "classification": {"classHierarchy": "Quantities / Environmental quantities / EPD EN 15804 / LCI indicators", "name": "GaBiCategories"}}, {"dataSetInternalID": 10, "referenceToFlowDataSet": {"shortDescription": [{"value": "Einsatz von Süßwasserressourcen (FW)", "lang": "de"}, {"value": "Use of net fresh water (FW)", "lang": "en"}], "type": "flow data set", "refObjectId": "3cf952c8-f3a4-461d-8c96-96456ca62246", "uri": "../flows/3cf952c8-f3a4-461d-8c96-96456ca62246.xml"}, "exchange direction": "INPUT", "other": {"anies": [{"name": "referenceToUnitGroupDataSet", "value": {"shortDescription": [{"value": "m^3", "lang": "de"}], "type": "unit group data set", "refObjectId": "cd950537-0a98-4044-9ba7-9f9a68d0a504", "uri": "../unitgroups/cd950537-0a98-4044-9ba7-9f9a68d0a504.xml"}}, {"value": "0.0357957856026909", "module": "A1-A3"}, {"value": "0.000142781118504576", "module": "A4"}, {"value": "0.00221769162666297", "module": "A5"}, {"value": "0.00138901279204506", "module": "B2"}, {"value": "0.000317356965386567", "module": "C1"}, {"value": "7.06127741522327E-06", "module": "C2"}, {"value": "0.00595817898293775", "module": "C3"}, {"value": "-0.00433938872754694", "module": "D"}]}, "resolvedFlowVersion": "38.00.000", "flowProperties": [], "typeOfFlow": "Other flow", "classification": {"classHierarchy": "Quantities / Environmental quantities / EPD EN 15804 / LCI indicators", "name": "GaBiCategories"}}, {"dataSetInternalID": 11, "referenceToFlowDataSet": {"shortDescription": [{"value": "Gefährlicher Abfall zur Deponie (HWD)", "lang": "de"}, {"value": "Hazardous waste disposed (HWD)", "lang": "en"}], "type": "flow data set", "refObjectId": "430f9e0f-59b2-46a0-8e0d-55e0e84948fc", "uri": "../flows/430f9e0f-59b2-46a0-8e0d-55e0e84948fc.xml"}, "exchange direction": "OUTPUT", "other": {"anies": [{"name": "referenceToUnitGroupDataSet", "value": {"shortDescription": [{"value": "kg", "lang": "de"}], "type": "unit group data set", "refObjectId": "ad38d542-3fe9-439d-9b95-2f5f7752acaf", "uri": "../unitgroups/ad38d542-3fe9-439d-9b95-2f5f7752acaf.xml"}}, {"value": "5.71543506846483E-05", "module": "A1-A3"}, {"value": "1.15489316961271E-10", "module": "A4"}, {"value": "2.95191592512274E-06", "module": "A5"}, {"value": "0.000413866975159284", "module": "B2"}, {"value": "1.86994608075474E-10", "module": "C1"}, {"value": "5.66618674714663E-12", "module": "C2"}, {"value": "8.48950655851696E-11", "module": "C3"}, {"value": "-4.39708567292115E-09", "module": "D"}]}, "resolvedFlowVersion": "38.00.000", "flowProperties": [], "typeOfFlow": "Other flow", "classification": {"classHierarchy": "Quantities / Environmental quantities / EPD EN 15804 / LCI indicators", "name": "GaBiCategories"}}, {"dataSetInternalID": 12, "referenceToFlowDataSet": {"shortDescription": [{"value": "Entsorgter nicht gefährlicher Abfall (NHWD)", "lang": "de"}, {"value": "Non hazardous waste disposed (NHWD)", "lang": "en"}], "type": "flow data set", "refObjectId": "b29ef66b-e286-4afa-949f-62f1a7b4d7fa", "uri": "../flows/b29ef66b-e286-4afa-949f-62f1a7b4d7fa.xml"}, "exchange direction": "OUTPUT", "other": {"anies": [{"name": "referenceToUnitGroupDataSet", "value": {"shortDescription": [{"value": "kg", "lang": "de"}], "type": "unit group data set", "refObjectId": "ad38d542-3fe9-439d-9b95-2f5f7752acaf", "uri": "../unitgroups/ad38d542-3fe9-439d-9b95-2f5f7752acaf.xml"}}, {"value": "3.10283988872558", "module": "A1-A3"}, {"value": "0.000365167541266479", "module": "A4"}, {"value": "0.165254975134215", "module": "A5"}, {"value": "0.0179808363398907", "module": "B2"}, {"value": "0.0005015896700272", "module": "C1"}, {"value": "1.68707638271156E-05", "module": "C2"}, {"value": "0.089015958333281", "module": "C3"}, {"value": "-0.0091987458277309", "module": "D"}]}, "resolvedFlowVersion": "38.00.000", "flowProperties": [], "typeOfFlow": "Other flow", "classification": {"classHierarchy": "Quantities / Environmental quantities / EPD EN 15804 / LCI indicators", "name": "GaBiCategories"}}, {"dataSetInternalID": 13, "referenceToFlowDataSet": {"shortDescription": [{"value": "Entsorgter radioaktiver Abfall (RWD)", "lang": "de"}, {"value": "Radioactive waste disposed (RWD)", "lang": "en"}], "type": "flow data set", "refObjectId": "3449546e-52ad-4b39-b809-9fb77cea8ff6", "uri": "../flows/3449546e-52ad-4b39-b809-9fb77cea8ff6.xml"}, "exchange direction": "OUTPUT", "other": {"anies": [{"name": "referenceToUnitGroupDataSet", "value": {"shortDescription": [{"value": "kg", "lang": "de"}], "type": "unit group data set", "refObjectId": "ad38d542-3fe9-439d-9b95-2f5f7752acaf", "uri": "../unitgroups/ad38d542-3fe9-439d-9b95-2f5f7752acaf.xml"}}, {"value": "0.00140131379690188", "module": "A1-A3"}, {"value": "4.21117660152341E-06", "module": "A4"}, {"value": "7.41457260866997E-05", "module": "A5"}, {"value": "0.000206277041047585", "module": "B2"}, {"value": "0.000105332077131332", "module": "C1"}, {"value": "1.95058331064946E-07", "module": "C2"}, {"value": "2.58832932567534E-05", "module": "C3"}, {"value": "-0.00142954004105486", "module": "D"}]}, "resolvedFlowVersion": "38.00.000", "flowProperties": [], "typeOfFlow": "Other flow", "classification": {"classHierarchy": "Quantities / Environmental quantities / EPD EN 15804 / LCI indicators", "name": "GaBiCategories"}}, {"dataSetInternalID": 14, "referenceToFlowDataSet": {"shortDescription": [{"value": "Komponenten für die Wiederverwendung (CRU)", "lang": "de"}, {"value": "Components for re-use (CRU)", "lang": "en"}], "type": "flow data set", "refObjectId": "a2b32f97-3fc7-4af2-b209-525bc6426f33", "uri": "../flows/a2b32f97-3fc7-4af2-b209-525bc6426f33.xml"}, "exchange direction": "OUTPUT", "other": {"anies": [{"name": "referenceToUnitGroupDataSet", "value": {"shortDescription": [{"value": "kg", "lang": "de"}], "type": "unit group data set", "refObjectId": "ad38d542-3fe9-439d-9b95-2f5f7752acaf", "uri": "../unitgroups/ad38d542-3fe9-439d-9b95-2f5f7752acaf.xml"}}, {"value": "0", "module": "A1-A3"}, {"value": "0", "module": "A4"}, {"value": "0", "module": "A5"}, {"value": "0", "module": "B2"}, {"value": "0", "module": "C1"}, {"value": "0", "module": "C2"}, {"value": "0", "module": "C3"}, {"value": "0", "module": "D"}]}, "resolvedFlowVersion": "38.00.000", "flowProperties": [], "typeOfFlow": "Other flow", "classification": {"classHierarchy": "Quantities / Environmental quantities / EPD EN 15804 / LCI indicators", "name": "GaBiCategories"}}, {"dataSetInternalID": 15, "referenceToFlowDataSet": {"shortDescription": [{"value": "Stoffe zum Recycling (MFR)", "lang": "de"}, {"value": "Materials for recycling (MFR)", "lang": "en"}], "type": "flow data set", "refObjectId": "d7fe48a5-4103-49c8-9aae-b0b5dfdbd6ae", "uri": "../flows/d7fe48a5-4103-49c8-9aae-b0b5dfdbd6ae.xml"}, "exchange direction": "OUTPUT", "other": {"anies": [{"name": "referenceToUnitGroupDataSet", "value": {"shortDescription": [{"value": "kg", "lang": "de"}], "type": "unit group data set", "refObjectId": "ad38d542-3fe9-439d-9b95-2f5f7752acaf", "uri": "../unitgroups/ad38d542-3fe9-439d-9b95-2f5f7752acaf.xml"}}, {"value": "0", "module": "A1-A3"}, {"value": "0", "module": "A4"}, {"value": "0.1", "module": "A5"}, {"value": "0", "module": "B2"}, {"value": "0", "module": "C1"}, {"value": "0", "module": "C2"}, {"value": "0", "module": "C3"}, {"value": "0", "module": "D"}]}, "resolvedFlowVersion": "38.00.000", "flowProperties": [], "typeOfFlow": "Other flow", "classification": {"classHierarchy": "Quantities / Environmental quantities / EPD EN 15804 / LCI indicators", "name": "GaBiCategories"}}, {"dataSetInternalID": 16, "referenceToFlowDataSet": {"shortDescription": [{"value": "Stoffe für die Energierückgewinnung (MER)", "lang": "de"}, {"value": "Materials for energy recovery (MER)", "lang": "en"}], "type": "flow data set", "refObjectId": "59a9181c-3aaf-46ee-8b13-2b3723b6e447", "uri": "../flows/59a9181c-3aaf-46ee-8b13-2b3723b6e447.xml"}, "exchange direction": "OUTPUT", "other": {"anies": [{"name": "referenceToUnitGroupDataSet", "value": {"shortDescription": [{"value": "kg", "lang": "de"}], "type": "unit group data set", "refObjectId": "ad38d542-3fe9-439d-9b95-2f5f7752acaf", "uri": "../unitgroups/ad38d542-3fe9-439d-9b95-2f5f7752acaf.xml"}}, {"value": "0", "module": "A1-A3"}, {"value": "0", "module": "A4"}, {"value": "0", "module": "A5"}, {"value": "0", "module": "B2"}, {"value": "0", "module": "C1"}, {"value": "0", "module": "C2"}, {"value": "0", "module": "C3"}, {"value": "0", "module": "D"}]}, "resolvedFlowVersion": "38.00.000", "flowProperties": [], "typeOfFlow": "Other flow", "classification": {"classHierarchy": "Quantities / Environmental quantities / EPD EN 15804 / LCI indicators", "name": "GaBiCategories"}}, {"dataSetInternalID": 17, "referenceToFlowDataSet": {"shortDescription": [{"value": "Exportierte elektrische Energie (EEE)", "lang": "de"}, {"value": "Exported electrical energy (EEE)", "lang": "en"}], "type": "flow data set", "refObjectId": "4da0c987-2b76-40d6-9e9e-82a017aaaf29", "uri": "../flows/4da0c987-2b76-40d6-9e9e-82a017aaaf29.xml"}, "exchange direction": "OUTPUT", "other": {"anies": [{"name": "referenceToUnitGroupDataSet", "value": {"shortDescription": [{"value": "MJ", "lang": "de"}], "type": "unit group data set", "refObjectId": "93a60a57-a3c8-11da-a746-0800200c9a66", "uri": "../unitgroups/93a60a57-a3c8-11da-a746-0800200c9a66.xml"}}, {"value": "0", "module": "A1-A3"}, {"value": "0", "module": "A4"}, {"value": "0.281", "module": "A5"}, {"value": "0", "module": "B2"}, {"value": "0", "module": "C1"}, {"value": "0", "module": "C2"}, {"value": "4.59", "module": "C3"}, {"value": "0", "module": "D"}]}, "resolvedFlowVersion": "38.00.000", "flowProperties": [], "typeOfFlow": "Other flow", "classification": {"classHierarchy": "Quantities / Environmental quantities / EPD EN 15804 / LCI indicators", "name": "GaBiCategories"}}, {"dataSetInternalID": 18, "referenceToFlowDataSet": {"shortDescription": [{"value": "Exportierte thermische Energie (EET)", "lang": "de"}, {"value": "Exported thermal energy (EET)", "lang": "en"}], "type": "flow data set", "refObjectId": "98daf38a-7a79-46d3-9a37-2b7bd0955810", "uri": "../flows/98daf38a-7a79-46d3-9a37-2b7bd0955810.xml"}, "exchange direction": "OUTPUT", "other": {"anies": [{"name": "referenceToUnitGroupDataSet", "value": {"shortDescription": [{"value": "MJ", "lang": "de"}], "type": "unit group data set", "refObjectId": "93a60a57-a3c8-11da-a746-0800200c9a66", "uri": "../unitgroups/93a60a57-a3c8-11da-a746-0800200c9a66.xml"}}, {"value": "0", "module": "A1-A3"}, {"value": "0", "module": "A4"}, {"value": "0.504", "module": "A5"}, {"value": "0", "module": "B2"}, {"value": "0", "module": "C1"}, {"value": "0", "module": "C2"}, {"value": "8.23", "module": "C3"}, {"value": "0", "module": "D"}]}, "resolvedFlowVersion": "38.00.000", "flowProperties": [], "typeOfFlow": "Other flow", "classification": {"classHierarchy": "Quantities / Environmental quantities / EPD EN 15804 / LCI indicators", "name": "GaBiCategories"}}]}, "LCIAResults": {"LCIAResult": [{"referenceToLCIAMethodDataSet": {"shortDescription": [{"value": "Globales Erwärmungspotenzial total (GWP-total)", "lang": "de"}, {"value": "Global Warming Potential total (GWP-total)", "lang": "en"}], "type": "LCIA method data set", "refObjectId": "6a37f984-a4b3-458a-a20a-64418c145fa2", "uri": "../lciamethods/6a37f984-a4b3-458a-a20a-64418c145fa2.xml"}, "other": {"anies": [{"name": "referenceToUnitGroupDataSet", "value": {"shortDescription": [{"value": "kg CO_(2)-Äq.", "lang": "de"}], "type": "unit group data set", "refObjectId": "1ebf3012-d0db-4de2-aefd-ef30cedb0be1", "uri": "../unitgroups/1ebf3012-d0db-4de2-aefd-ef30cedb0be1.xml"}}, {"value": "9.48293225690573", "module": "A1-A3"}, {"value": "0.185623453528195", "module": "A4"}, {"value": "0.677597954600911", "module": "A5"}, {"value": "0.355314065238847", "module": "B2"}, {"value": "0.040144418312565", "module": "C1"}, {"value": "0.00812021748687008", "module": "C2"}, {"value": "2.96550520910842", "module": "C3"}, {"value": "-1.13250083933533", "module": "D"}]}}, {"referenceToLCIAMethodDataSet": {"shortDescription": [{"value": "Globales Erwärmungspotenzial fossil (GWP-fossil)", "lang": "de"}, {"value": "Global Warming Potential fossil fuels (GWP-fossil)", "lang": "en"}], "type": "LCIA method data set", "refObjectId": "5f635281-343e-44fb-83df-1971b155e6b6", "uri": "../lciamethods/5f635281-343e-44fb-83df-1971b155e6b6.xml"}, "other": {"anies": [{"name": "referenceToUnitGroupDataSet", "value": {"shortDescription": [{"value": "kg CO_(2)-Äq.", "lang": "de"}], "type": "unit group data set", "refObjectId": "1ebf3012-d0db-4de2-aefd-ef30cedb0be1", "uri": "../unitgroups/1ebf3012-d0db-4de2-aefd-ef30cedb0be1.xml"}}, {"value": "9.36053202423044", "module": "A1-A3"}, {"value": "0.184470138555789", "module": "A4"}, {"value": "0.66654768292031", "module": "A5"}, {"value": "0.345064496420859", "module": "B2"}, {"value": "0.0397501978896218", "module": "C1"}, {"value": "0.00806404835349323", "module": "C2"}, {"value": "2.96534969511103", "module": "C3"}, {"value": "-1.12606838171483", "module": "D"}]}}, {"referenceToLCIAMethodDataSet": {"shortDescription": [{"value": "Globales Erwärmungspotenzial biogen (GWP-biogenic)", "lang": "de"}, {"value": "Global Warming Potential biogenic (GWP-biogenic)", "lang": "en"}], "type": "LCIA method data set", "refObjectId": "2356e1ab-0185-4db5-86e5-16de51c7485c", "uri": "../lciamethods/2356e1ab-0185-4db5-86e5-16de51c7485c.xml"}, "other": {"anies": [{"name": "referenceToUnitGroupDataSet", "value": {"shortDescription": [{"value": "kg CO_(2)-Äq.", "lang": "de"}], "type": "unit group data set", "refObjectId": "1ebf3012-d0db-4de2-aefd-ef30cedb0be1", "uri": "../unitgroups/1ebf3012-d0db-4de2-aefd-ef30cedb0be1.xml"}}, {"value": "-0.00343217994444185", "module": "A1-A3"}, {"value": "0", "module": "A4"}, {"value": "0.00448141084318789", "module": "A5"}, {"value": "0.0102006182413728", "module": "B2"}, {"value": "0.000337935458070473", "module": "C1"}, {"value": "0", "module": "C2"}, {"value": "0.000122223900268944", "module": "C3"}, {"value": "-0.00565020933735865", "module": "D"}]}}, {"referenceToLCIAMethodDataSet": {"shortDescription": [{"value": "Globales Erwärmungspotenzial luluc (GWP-luluc)", "lang": "de"}, {"value": "Global Warming Potential luluc (GWP-luluc)", "lang": "en"}], "type": "LCIA method data set", "refObjectId": "4331bbdb-978a-490d-8707-eeb047f01a55", "uri": "../lciamethods/4331bbdb-978a-490d-8707-eeb047f01a55.xml"}, "other": {"anies": [{"name": "referenceToUnitGroupDataSet", "value": {"shortDescription": [{"value": "kg CO_(2)-Äq.", "lang": "de"}], "type": "unit group data set", "refObjectId": "1ebf3012-d0db-4de2-aefd-ef30cedb0be1", "uri": "../unitgroups/1ebf3012-d0db-4de2-aefd-ef30cedb0be1.xml"}}, {"value": "0.125832412619732", "module": "A1-A3"}, {"value": "0.00131547283645839", "module": "A4"}, {"value": "0.00656886083741285", "module": "A5"}, {"value": "4.89505766157058E-05", "module": "B2"}, {"value": "5.62849648727753E-05", "module": "C1"}, {"value": "6.57501025685248E-05", "module": "C2"}, {"value": "3.32900971222342E-05", "module": "C3"}, {"value": "-0.000782248283148538", "module": "D"}]}}, {"referenceToLCIAMethodDataSet": {"shortDescription": [{"value": "Abbau Potential der stratosphärischen Ozonschicht (ODP)", "lang": "de"}, {"value": "Depletion potential of the stratospheric ozone layer (ODP)", "lang": "en"}], "type": "LCIA method data set", "refObjectId": "b5c629d6-def3-11e6-bf01-fe55135034f3", "uri": "../lciamethods/b5c629d6-def3-11e6-bf01-fe55135034f3.xml"}, "other": {"anies": [{"name": "referenceToUnitGroupDataSet", "value": {"shortDescription": [{"value": "kg CFC11-Äq.", "lang": "de"}], "type": "unit group data set", "refObjectId": "d9e957c9-7309-4474-bf3a-7777df6c4e5b", "uri": "../unitgroups/d9e957c9-7309-4474-bf3a-7777df6c4e5b.xml"}}, {"value": "2.11194586072628E-08", "module": "A1-A3"}, {"value": "3.41301780097157E-17", "module": "A4"}, {"value": "1.09077669949361E-09", "module": "A5"}, {"value": "2.68814802663477E-11", "module": "B2"}, {"value": "9.51741155464629E-16", "module": "C1"}, {"value": "1.58811413148952E-18", "module": "C2"}, {"value": "3.0313257188115E-16", "module": "C3"}, {"value": "-1.29314894728911E-14", "module": "D"}]}}, {"referenceToLCIAMethodDataSet": {"shortDescription": [{"value": "Versauerungspotenzial von Boden und Wasser (AP)", "lang": "de"}, {"value": "Acidification potential of land and water (AP)", "lang": "en"}], "type": "LCIA method data set", "refObjectId": "b5c611c6-def3-11e6-bf01-fe55135034f3", "uri": "../lciamethods/b5c611c6-def3-11e6-bf01-fe55135034f3.xml"}, "other": {"anies": [{"name": "referenceToUnitGroupDataSet", "value": {"shortDescription": [{"value": "mol H^(+)-Äq.", "lang": "de"}], "type": "unit group data set", "refObjectId": "42e089ac-92bf-4bf2-8ca1-5fc40d18f2ed", "uri": "../unitgroups/42e089ac-92bf-4bf2-8ca1-5fc40d18f2ed.xml"}}, {"value": "0.0391116443487538", "module": "A1-A3"}, {"value": "0.00137115401682727", "module": "A4"}, {"value": "0.00210848129806803", "module": "A5"}, {"value": "0.00101264156671095", "module": "B2"}, {"value": "8.27243735744765E-05", "module": "C1"}, {"value": "2.42387092764414E-05", "module": "C2"}, {"value": "0.000289499597128331", "module": "C3"}, {"value": "-0.00147565739704432", "module": "D"}]}}, {"referenceToLCIAMethodDataSet": {"shortDescription": [{"value": "Eutrophierungspotenzial Süßwasser (EP-freshwater)", "lang": "de"}, {"value": "Eutrophication potential aquatic freshwater (EP-freshwater)", "lang": "en"}], "type": "LCIA method data set", "refObjectId": "b53ec18f-7377-4ad3-86eb-cc3f4f276b2b", "uri": "../lciamethods/b53ec18f-7377-4ad3-86eb-cc3f4f276b2b.xml"}, "other": {"anies": [{"name": "referenceToUnitGroupDataSet", "value": {"shortDescription": [{"value": "kg PO_(4)-Äq.", "lang": "de"}], "type": "unit group data set", "refObjectId": "0429039d-a61d-4590-ba67-aa4a20a810a1", "uri": "../unitgroups/0429039d-a61d-4590-ba67-aa4a20a810a1.xml"}}, {"value": "3.98405726593149E-05", "module": "A1-A3"}, {"value": "4.83150776210917E-07", "module": "A4"}, {"value": "2.08701948814297E-06", "module": "A5"}, {"value": "1.09326791566053E-05", "module": "B2"}, {"value": "1.06643889068288E-07", "module": "C1"}, {"value": "2.38978451414508E-08", "module": "C2"}, {"value": "7.61323032771959E-08", "module": "C3"}, {"value": "-1.47941251256559E-06", "module": "D"}]}}, {"referenceToLCIAMethodDataSet": {"shortDescription": [{"value": "Eutrophierungspotenzial Salzwasser (EP-marine)", "lang": "de"}, {"value": "Eutrophication potential aquatic marine (EP-marine)", "lang": "en"}], "type": "LCIA method data set", "refObjectId": "b5c619fa-def3-11e6-bf01-fe55135034f3", "uri": "../lciamethods/b5c619fa-def3-11e6-bf01-fe55135034f3.xml"}, "other": {"anies": [{"name": "referenceToUnitGroupDataSet", "value": {"shortDescription": [{"value": "kg N-Äq.", "lang": "de"}], "type": "unit group data set", "refObjectId": "d05bb823-ecdf-4686-8c40-bf1d9257859f", "uri": "../unitgroups/d05bb823-ecdf-4686-8c40-bf1d9257859f.xml"}}, {"value": "0.0105782276491927", "module": "A1-A3"}, {"value": "0.000445069434134021", "module": "A4"}, {"value": "0.000573913133895743", "module": "A5"}, {"value": "0.000218632457531444", "module": "B2"}, {"value": "1.96509088288847E-05", "module": "C1"}, {"value": "1.09767728333477E-05", "module": "C2"}, {"value": "7.53315769260332E-05", "module": "C3"}, {"value": "-0.000418999657080493", "module": "D"}]}}, {"referenceToLCIAMethodDataSet": {"shortDescription": [{"value": "Eutrophierungspotenzial Land (EP-terrestrial)", "lang": "de"}, {"value": "Eutrophication potential terrestrial (EP-terrestrial)", "lang": "en"}], "type": "LCIA method data set", "refObjectId": "b5c614d2-def3-11e6-bf01-fe55135034f3", "uri": "../lciamethods/b5c614d2-def3-11e6-bf01-fe55135034f3.xml"}, "other": {"anies": [{"name": "referenceToUnitGroupDataSet", "value": {"shortDescription": [{"value": "mol N-Äq.", "lang": "de"}], "type": "unit group data set", "refObjectId": "71b4d617-0ec9-4d3f-b65e-e438940c2401", "uri": "../unitgroups/71b4d617-0ec9-4d3f-b65e-e438940c2401.xml"}}, {"value": "0.113725345853733", "module": "A1-A3"}, {"value": "0.00492510178310732", "module": "A4"}, {"value": "0.00621075944483449", "module": "A5"}, {"value": "0.00193324281896639", "module": "B2"}, {"value": "0.000206311257656362", "module": "C1"}, {"value": "0.000122755841966539", "module": "C2"}, {"value": "0.00135742261590913", "module": "C3"}, {"value": "-0.00448810513478543", "module": "D"}]}}, {"referenceToLCIAMethodDataSet": {"shortDescription": [{"value": "Bildungspotential für troposphärisches Ozon (POCP)", "lang": "de"}, {"value": "Formation potential of tropospheric ozone photochemical oxidants (POCP)", "lang": "en"}], "type": "LCIA method data set", "refObjectId": "b5c610fe-def3-11e6-bf01-fe55135034f3", "uri": "../lciamethods/b5c610fe-def3-11e6-bf01-fe55135034f3.xml"}, "other": {"anies": [{"name": "referenceToUnitGroupDataSet", "value": {"shortDescription": [{"value": "kg NMVOC-Äq.", "lang": "de"}], "type": "unit group data set", "refObjectId": "d27c25f8-fbc1-44c6-b47b-4adbae4199c6", "uri": "../unitgroups/d27c25f8-fbc1-44c6-b47b-4adbae4199c6.xml"}}, {"value": "0.0324979336943906", "module": "A1-A3"}, {"value": "0.00106873119705504", "module": "A4"}, {"value": "0.00174671904148133", "module": "A5"}, {"value": "0.00100377584659266", "module": "B2"}, {"value": "5.33221655442072E-05", "module": "C1"}, {"value": "2.18150022077199E-05", "module": "C2"}, {"value": "0.000214919196375097", "module": "C3"}, {"value": "-0.00117612206342622", "module": "D"}]}}, {"referenceToLCIAMethodDataSet": {"shortDescription": [{"value": "Potenzial für den abiotischen Abbau nicht fossiler Ressourcen (ADPE)", "lang": "de"}, {"value": "Abiotic depletion potential for non fossil resources (ADPE)", "lang": "en"}], "type": "LCIA method data set", "refObjectId": "b2ad6494-c78d-11e6-9d9d-cec0c932ce01", "uri": "../lciamethods/b2ad6494-c78d-11e6-9d9d-cec0c932ce01.xml"}, "other": {"anies": [{"name": "referenceToUnitGroupDataSet", "value": {"shortDescription": [{"value": "kg Sb-Äq.", "lang": "de"}], "type": "unit group data set", "refObjectId": "54ccd2d9-a32a-4fc2-923d-f2c8c93e89d4", "uri": "../unitgroups/54ccd2d9-a32a-4fc2-923d-f2c8c93e89d4.xml"}}, {"value": "0.000175863980214289", "module": "A1-A3"}, {"value": "1.49431660352315E-08", "module": "A4"}, {"value": "9.08406227857739E-06", "module": "A5"}, {"value": "6.29625100147254E-08", "module": "B2"}, {"value": "1.1696457126564E-08", "module": "C1"}, {"value": "7.12982942908542E-10", "module": "C2"}, {"value": "4.64763831115599E-09", "module": "C3"}, {"value": "-1.87950294929328E-07", "module": "D"}]}}, {"referenceToLCIAMethodDataSet": {"shortDescription": [{"value": "Potenzial für den abiotischen Abbau fossiler Brennstoffe (ADPF)", "lang": "de"}, {"value": "Abiotic depletion potential for fossil resources (ADPF)", "lang": "en"}], "type": "LCIA method data set", "refObjectId": "b2ad6110-c78d-11e6-9d9d-cec0c932ce01", "uri": "../lciamethods/b2ad6110-c78d-11e6-9d9d-cec0c932ce01.xml"}, "other": {"anies": [{"name": "referenceToUnitGroupDataSet", "value": {"shortDescription": [{"value": "MJ", "lang": "de"}], "type": "unit group data set", "refObjectId": "93a60a57-a3c8-11da-a746-0800200c9a66", "uri": "../unitgroups/93a60a57-a3c8-11da-a746-0800200c9a66.xml"}}, {"value": "194.822628820471", "module": "A1-A3"}, {"value": "2.41897926451625", "module": "A4"}, {"value": "10.2161395617994", "module": "A5"}, {"value": "8.05343606281901", "module": "B2"}, {"value": "0.707183994961737", "module": "C1"}, {"value": "0.107143540265251", "module": "C2"}, {"value": "0.485556479972777", "module": "C3"}, {"value": "-19.5460938024917", "module": "D"}]}}, {"referenceToLCIAMethodDataSet": {"shortDescription": [{"value": "Wassernutzung (WDP)", "lang": "de"}, {"value": "Water use (WDP)", "lang": "en"}], "type": "LCIA method data set", "refObjectId": "b2ad66ce-c78d-11e6-9d9d-cec0c932ce01", "uri": "../lciamethods/b2ad66ce-c78d-11e6-9d9d-cec0c932ce01.xml"}, "other": {"anies": [{"name": "referenceToUnitGroupDataSet", "value": {"shortDescription": [{"value": "m^(3) Welt-Äq. entzogen", "lang": "de"}], "type": "unit group data set", "refObjectId": "6ae2df01-888e-46c8-b17d-49fa3869b476", "uri": "../unitgroups/6ae2df01-888e-46c8-b17d-49fa3869b476.xml"}}, {"value": "0.304795867675546", "module": "A1-A3"}, {"value": "0.00152816134120763", "module": "A4"}, {"value": "0.0312119552495649", "module": "A5"}, {"value": "0.0536568730152851", "module": "B2"}, {"value": "0.00637937999718385", "module": "C1"}, {"value": "7.46460999240823E-05", "module": "C2"}, {"value": "0.253609866219794", "module": "C3"}, {"value": "-0.086769122611104", "module": "D"}]}}, {"referenceToLCIAMethodDataSet": {"shortDescription": [{"value": "Auftreten von Krankheiten aufgrund von Feinstaubemissionen (PM)", "lang": "de"}, {"value": "Incidence of disease due to PM emissions (PM)", "lang": "en"}], "type": "LCIA method data set", "refObjectId": "b5c602c6-def3-11e6-bf01-fe55135034f3", "uri": "../lciamethods/b5c602c6-def3-11e6-bf01-fe55135034f3.xml"}, "other": {"anies": [{"name": "referenceToUnitGroupDataSet", "value": {"shortDescription": [{"value": "Krankheitsfälle", "lang": "de"}], "type": "unit group data set", "refObjectId": "3883559b-648f-4afc-8ba2-0bd24f3affa3", "uri": "../unitgroups/3883559b-648f-4afc-8ba2-0bd24f3affa3.xml"}}, {"value": "5.35532340348483E-07", "module": "A1-A3"}, {"value": "1.76424109197865E-08", "module": "A4"}, {"value": "2.87314613782228E-08", "module": "A5"}, {"value": "1.29408864060531E-08", "module": "B2"}, {"value": "6.97572586265732E-10", "module": "C1"}, {"value": "1.42340162530531E-10", "module": "C2"}, {"value": "2.75458524672902E-09", "module": "C3"}, {"value": "-1.26917796401742E-08", "module": "D"}]}}, {"referenceToLCIAMethodDataSet": {"shortDescription": [{"value": "Wirkung durch Exposition des Menschen mit U235 (IR)", "lang": "de"}, {"value": "Human exposure efficiency relative to U235 (IR)", "lang": "en"}], "type": "LCIA method data set", "refObjectId": "b5c632be-def3-11e6-bf01-fe55135034f3", "uri": "../lciamethods/b5c632be-def3-11e6-bf01-fe55135034f3.xml"}, "other": {"anies": [{"name": "referenceToUnitGroupDataSet", "value": {"shortDescription": [{"value": "kBq U235-Äq.", "lang": "de"}], "type": "unit group data set", "refObjectId": "456b05bf-1415-44a9-9993-02452f554c09", "uri": "../unitgroups/456b05bf-1415-44a9-9993-02452f554c09.xml"}}, {"value": "0.173114560209661", "module": "A1-A3"}, {"value": "0.000614791104838648", "module": "A4"}, {"value": "0.00921538649106595", "module": "A5"}, {"value": "0.130488119496108", "module": "B2"}, {"value": "0.0172864507168269", "module": "C1"}, {"value": "2.85264823255461E-05", "module": "C2"}, {"value": "0.00403750241662744", "module": "C3"}, {"value": "-0.234479657448937", "module": "D"}]}}, {"referenceToLCIAMethodDataSet": {"shortDescription": [{"value": "Toxizitätsvergleichseinheit für Ökosysteme (ETP-fw)", "lang": "de"}, {"value": "Comparative toxic unit for ecosystems (ETP-fw)", "lang": "en"}], "type": "LCIA method data set", "refObjectId": "ee1082d1-b0f7-43ca-a1f0-21e2a4a74511", "uri": "../lciamethods/ee1082d1-b0f7-43ca-a1f0-21e2a4a74511.xml"}, "other": {"anies": [{"name": "referenceToUnitGroupDataSet", "value": {"shortDescription": [{"value": "CTUe", "lang": "de"}], "type": "unit group data set", "refObjectId": "aa959ded-f1eb-4efb-9c5c-2d60be36b3e6", "uri": "../unitgroups/aa959ded-f1eb-4efb-9c5c-2d60be36b3e6.xml"}}, {"value": "109.509886999395", "module": "A1-A3"}, {"value": "1.78972244335929", "module": "A4"}, {"value": "5.76367701393385", "module": "A5"}, {"value": "2.75590528071642", "module": "B2"}, {"value": "0.297388158792229", "module": "C1"}, {"value": "0.0795062400376562", "module": "C2"}, {"value": "0.259100173529202", "module": "C3"}, {"value": "-4.11373850858591", "module": "D"}]}}, {"referenceToLCIAMethodDataSet": {"shortDescription": [{"value": "Toxizitätsvergleichseinheit für Menschen (krebserregend) (HTP-c)", "lang": "de"}, {"value": "Comparative toxic unit for humans (carcinogenic) (HTP-c)", "lang": "en"}], "type": "LCIA method data set", "refObjectId": "2299222a-bbd8-474f-9d4f-4dd1f18aea7c", "uri": "../lciamethods/2299222a-bbd8-474f-9d4f-4dd1f18aea7c.xml"}, "other": {"anies": [{"name": "referenceToUnitGroupDataSet", "value": {"shortDescription": [{"value": "CTUh", "lang": "de"}], "type": "unit group data set", "refObjectId": "d4c9523e-2d7e-49fd-8469-998f547d3a70", "uri": "../unitgroups/d4c9523e-2d7e-49fd-8469-998f547d3a70.xml"}}, {"value": "3.41299154202278E-09", "module": "A1-A3"}, {"value": "3.58760301902822E-11", "module": "A4"}, {"value": "1.79215896798677E-10", "module": "A5"}, {"value": "8.92914898655281E-11", "module": "B2"}, {"value": "8.42314546393219E-12", "module": "C1"}, {"value": "1.60783710590285E-12", "module": "C2"}, {"value": "1.80487764529027E-11", "module": "C3"}, {"value": "-1.86418614362905E-10", "module": "D"}]}}, {"referenceToLCIAMethodDataSet": {"shortDescription": [{"value": "Toxizitätsvergleichseinheit für Menschen (nicht krebserregend) (HTP-nc)", "lang": "de"}, {"value": "Comparative toxic unit for humans (noncarcinogenic) (HTP-nc)", "lang": "en"}], "type": "LCIA method data set", "refObjectId": "3af763a5-b7a1-48c9-9cee-1f223481fcef", "uri": "../lciamethods/3af763a5-b7a1-48c9-9cee-1f223481fcef.xml"}, "other": {"anies": [{"name": "referenceToUnitGroupDataSet", "value": {"shortDescription": [{"value": "CTUh", "lang": "de"}], "type": "unit group data set", "refObjectId": "d4c9523e-2d7e-49fd-8469-998f547d3a70", "uri": "../unitgroups/d4c9523e-2d7e-49fd-8469-998f547d3a70.xml"}}, {"value": "2.09213797229103E-07", "module": "A1-A3"}, {"value": "2.04621328072103E-09", "module": "A4"}, {"value": "1.09540942045541E-08", "module": "A5"}, {"value": "1.56394760908557E-08", "module": "B2"}, {"value": "3.17753295173089E-10", "module": "C1"}, {"value": "9.36159764245212E-11", "module": "C2"}, {"value": "7.23079904847654E-10", "module": "C3"}, {"value": "-7.3581129353961E-09", "module": "D"}]}}, {"referenceToLCIAMethodDataSet": {"shortDescription": [{"value": "Bodenqualitätsindex (SQP)", "lang": "de"}, {"value": "Soil quality index (SQP)", "lang": "en"}], "type": "LCIA method data set", "refObjectId": "b2ad6890-c78d-11e6-9d9d-cec0c932ce01", "uri": "../lciamethods/b2ad6890-c78d-11e6-9d9d-cec0c932ce01.xml"}, "other": {"anies": [{"name": "referenceToUnitGroupDataSet", "value": {"shortDescription": [{"value": "SQP", "lang": "de"}], "type": "unit group data set", "refObjectId": "f130951c-e67f-4f7f-8dd4-665de3974e18", "uri": "../unitgroups/f130951c-e67f-4f7f-8dd4-665de3974e18.xml"}}, {"value": "24.5515877779147", "module": "A1-A3"}, {"value": "0.737260746579891", "module": "A4"}, {"value": "1.31426591247717", "module": "A5"}, {"value": "0.212482696703052", "module": "B2"}, {"value": "0.22314422658732", "module": "C1"}, {"value": "0.0368261579990573", "module": "C2"}, {"value": "0.136514021344417", "module": "C3"}, {"value": "-3.04093149896225", "module": "D"}]}}]}, "otherAttributes": {"{http://www.indata.network/EPD/2019}epd-version": "1.2"}, "version": "1.1", "locations": "../ILCDLocations.xml"}