{"processInformation": {"dataSetInformation": {"UUID": "f97a021b-82db-47d5-955f-d0afd04b23f9", "name": {"baseName": [{"value": "LIGNOLOC® HOLZNAGEL", "lang": "de"}, {"value": "LIGNOLOC® Wooden Nail", "lang": "en"}], "functionalUnitFlowProperties": [{"lang": "de"}]}, "classificationInformation": {"classification": [{"class": [{"value": "Holz", "level": 0, "classId": "3"}, {"value": "Holzwerkstoffe", "level": 1, "classId": "3.2"}, {"value": "Elemente aus Holzwerkstoffen", "level": 2, "classId": "3.2.10"}], "name": "OEKOBAU.DAT"}, {"class": [{"value": "02 Bauprodukte", "level": 0}, {"value": "Holzwerkstoffe", "level": 1}, {"value": "Holzwerkstoffe", "level": 2}], "name": "IBUCategories"}]}, "generalComment": [{"value": "Die LignoLoc® Produktlinie umfasst holzgefertigte stiftfrmige Verbindungsmittel, zur Befestigung von zwei Holzwerkstoff-Bauteilen, die fr verschiedene Anwendungen in der Holzbauindustrie entwickelt wurden. \n\nDie Holzngel sind auf einem Kunststoffband magaziniert, auch Magazinierungsband genannt, und knnen somit mit einem Druckluftgert verarbeitet werden. Die Ngel sind zur Herstellung von Holz-Holz- oder Platten-Holz-Verbindungen in tragenden, aussteifenden oder mittragenden Holzkonstruktionen mit Bauteilen aus Nadelholz, z. B. Vollholz, Brettschichtholz, Brettsperrholz, Furnierschichtholz und hnlich verleimten Bauteilen, Holzwerkstoffen oder Gipsfaserplatten bestimmt.\n\nDie Ngel bestehen aus verdichtetem Buchenschichtholz und sind in unterschiedlichen Varianten erhltlich. Der LignoLoc® Holznagel kann mit Kopf, ohne Kopf, eine Profilierung, eine Abstufung am Schaft, eine abgestumpfte oder unterschiedlich ausgeformte Spitze aufweisen. Je nach Anwendung kann das Verbindungsmittel unterschiedliche geometrische Eigenschaften aufweisen. \n\nDie deklarierte Einheit von 1 kg Holznagel enthlt eine durchschnittliche Anzahl von 537 Ngeln.", "lang": "de"}, {"value": "The LignoLoc® line of products consists of pin-type fasteners made of wood and intended to connect two wood-based components which were designed for various applications in the timber construction industry.\n\nThe wooden nails are collated on a plastic band also called collation band so that they can be processed using a compressed air tool. The nails are intended for use in wood-wood or board-wood connections in load-bearing or stiffening timber structures or timber structures contributing to load-bearing with softwood elements, e.g., solid timber, glue-laminated timber, cross-laminated timber, laminated veneer timber, and similarly glued components, wood-based materials or gypsum fibreboard.\n\nThe nails are made of densified, laminated beech wood, and come in different variants. The LignoLoc® wooden nail comes with head, without head, with profile, stepped shaft, a blunt or differently shaped point. Depending on the application, the fastener can have varying geometric properties.\n\nThe declared unit of 1 kg of wooden nails consists of 537 nails on average.", "lang": "en"}]}, "quantitativeReference": {"referenceToReferenceFlow": [0]}, "time": {"referenceYear": 2024, "dataSetValidUntil": 2029, "other": {"anies": [{"name": "publicationDateOfEPD", "value": 1734652800000}]}}, "geography": {"locationOfOperationSupplyOrProduction": {"location": "DE"}}, "technology": {"technologyDescriptionAndIncludedProcesses": [{"value": "Die LIGNOLOC® Produktlinie umfasst holzgefertigte stiftförmige Verbindungsmittel, zur Befestigung von zwei Holzwerkstoff-Bauteilen, die für verschiedene Anwendungen in der Holzbauindustrie entwickelt wurden. Hierfür kann ein Druckluftgerät zum Eintreiben des LIGNOLOC Holznagels verwendet werden. Die Nägel sind zur Herstellung von Holz-Holz- oder Platten-Holz-Verbindungen in tragenden, aussteifenden oder mittragenden Holzkonstruktionen mit Bauteilen aus Nadelholz, z. B. Vollholz, Brettschichtholz, Brettsperrholz, Furnierschichtholz und ähnlich verleimten Bauteilen, Holzwerkstoffen oder Gipsfaserplatten bestimmt. Diese Nägel bestehen aus verdichtetem Buchenschichtholz und sind in unterschiedlichen Varianten erhältlich. Je nach Anwendung kann das Verbindungmittel unterschiedliche geometrische Eigenschaften aufweisen. Der LIGNOLOC Holznagel kann mit Kopf, ohne Kopf, eine Profilierung, eine Abstufung am Schaft, eine abgestumpfte oder unterschiedlich ausgeformte Spitze aufweisen. \nTechnische Daten: \nBautechnische Daten zum Holznagel LignoLoc® sind in den entsprechenden Zulassungen sowie technischen Zeichnungen hinterlegt, nachfolgend beispielhaft dargestellt an einem Auszug aus der ETA 23-0041 und ETA 23-0330 fr Holzngel. \nDeklarierte Einheit: \nAls Referenz dieser Deklaration dient 1 kg Holznagel Lignoloc® (magaziniert zu Rollen, sog. Coils).", "lang": "de"}, {"value": "Die LIGNOLOC® Produktlinie umfasst holzgefertigte stiftförmige Verbindungsmittel, zur Befestigung von zwei Holzwerkstoff-Bauteilen, die für verschiedene Anwendungen in der Holzbauindustrie entwickelt wurden. Hierfür kann ein Druckluftgerät zum Eintreiben des LIGNOLOC Holznagels verwendet werden. Die Nägel sind zur Herstellung von Holz-Holz- oder Platten-Holz-Verbindungen in tragenden, aussteifenden oder mittragenden Holzkonstruktionen mit Bauteilen aus Nadelholz, z. B. Vollholz, Brettschichtholz, Brettsperrholz, Furnierschichtholz und ähnlich verleimten Bauteilen, Holzwerkstoffen oder Gipsfaserplatten bestimmt. Diese Nägel bestehen aus verdichtetem Buchenschichtholz und sind in unterschiedlichen Varianten erhältlich. Je nach Anwendung kann das Verbindungmittel unterschiedliche geometrische Eigenschaften aufweisen. Der LIGNOLOC Holznagel kann mit Kopf, ohne Kopf, eine Profilierung, eine Abstufung am Schaft, eine abgestumpfte oder unterschiedlich ausgeformte Spitze aufweisen. \nTechnical data: \nConstructional data of the LignoLoc® wooden nail can be found in the respective approvals and technical drawings, as exemplified by the following extract from ETA 23-0041 and ETA 23-0330 for wooden nails. \nDeclared unit: \n1 kg of LignoLoc® wood nails (collated into coils) are used as reference for this declaration.", "lang": "en"}], "technologicalApplicability": [{"value": "Die Ngel sind zur Herstellung von Holz-Holz oder Platten-Holz-Verbindungen in tragenden Holzkonstruktionen mit Bauteilen aus: \nNadelsperrholz gem EN 636 oder Europischer Technischer Bewertung (Mindestrohdichte 400 kg/m und Hchstrohdichte 700 kg/m) \nGrobspanplatten OSB/3 und OSB/4 gem EN 300 oder Europischer Technischer Bewertung (Mindestdichte 500 kg/m und Hchstrohdichte 700 kg/m) \nFaserplatten gem EN 622-5 und EN 13986 oder Europischer Technischer Bewertung (Mindestrohdichte 500 kg/m und Hchstrohdichte 700 kg/m, nur fr Nutzungsklasse 1) \nVollholzplatten gem EN 13353 und EN 13986 oder Europischer Technischer Bewertung (Mindestrohdichte 400 kg/m und Hchstrohdichte 700 kg/m) \nGipsfaserplatten gem Europischer Technischer Bewertung oder EAD Nr. 070006-00-050415 (Mindestrohdichte 1050 kg/m und Hchstrohdichte 1250 kg/m, nur fr Nutzungsklasse 1), bestimmt. Die Ngel sind ohne Vorbohren senkrecht zur Faserrichtung in das Holz mit einem Druckluftgert einzutreiben. Hierbei ist die Hchstrohdichte der Holzstoffe zu beachten. Bei Hlzern mit einer hohen Rohdichte wird das Vorbohren empfohlen. Die Ngel sind zur Verwendung in Verbindungen mit statischer oder quasistatischer Beanspruchung vorgesehen.", "lang": "de"}, {"value": "The nails are intended for the production of wood-wood or board-wood connections in load-bearing constructions with elements made of:\n Softwood plywood acc. to EN 636 or European Technical Assessment (minimum bulk density 400 kg/m, maximum bulk density 700 kg/m)\nOriented strand board OSB/3 und OSB/4 acc. to EN 300 or European Technical Assessment (minimum bulk density 500 kg/m, maximum bulk density 700 kg/m)\nFibreboard acc. to EN 622-5 and EN 13986 or European Technical Assessment (minimum bulk density 500 kg/m, maximum bulk density 700 kg/m, only for service class 1)\nSolid timber board acc. to EN 13353 and EN 13986 or European Technical Assessment (minimum bulk density 400 kg/m, maximum bulk density 700 kg/m)\nGypsum fibreboard acc. to European Technical Assessment or EAD no. 07000600050415 (minimum bulk density 1050 kg/m, maximum bulk density 1250 kg/m, only for service class 1). \n\nThe nails are supposed to be driven into the wood without pre-drilling perpendicularly to the direction of the fibres using a compressed air tool, taking account of the maximum bulk density of the wood materials. Pre-drilling is recommended for high-bulk density wood. The nails are intended for use in connections which are subject to static or quasi-static loads.", "lang": "en"}]}}, "modellingAndValidation": {"LCIMethodAndAllocation": {"typeOfDataSet": "EPD", "referenceToLCAMethodDetails": [{"shortDescription": [{"value": "Holzwerkstoffe.pdf", "lang": "de"}], "type": "source data set", "refObjectId": "1fb480ff-c34b-42b7-8a53-beec3ad9eceb"}], "other": {"anies": [{"name": "subType", "value": "specific dataset"}]}}, "dataSourcesTreatmentAndRepresentativeness": {"referenceToDataSource": [{"shortDescription": [{"value": "GaBi Database (all versions)", "lang": "de"}], "type": "source data set", "refObjectId": "28d74cc0-db8b-4d7e-bc44-5f6d56ce0c4a"}, {"shortDescription": [{"value": "Sphera MLC (fka GaBi) CUP 2023.02", "lang": "de"}], "type": "source data set", "refObjectId": "cb600d3b-e85a-42b3-b059-5591e2757fbb"}], "useAdviceForDataSet": [{"value": "Gültigkeitsbereich: \nDie Ngel sind zur Herstellung von Holz-Holz- oder Platten-Holz-Verbindungen in tragenden, aussteifenden oder mittragenden Holzkonstruktionen mit Bauteilen aus Nadelholz, z. B. Vollholz, Brettschichtholz, Brettsperrholz, Furnierschichtholz und hnlich verleimten Bauteilen, Holzwerkstoffen oder Gipsfaserplatten bestimmt.\n\nDie deklarierten Umweltdaten bezogen auf 1 kg LignoLoc® Holznagel basieren auf einem gewichteten Durchschnitt von Holzngeln der Raimund BECK Nageltechnik GmbH, im Herstellwerk Mauerkirchen, AT und sind mit generischen Daten fr Deutschland und sterreich regionalisiert. \nSystemgrenze: \nDer Deklarationstyp entspricht einer EPD Wiege bis Werkstor – mit Optionen. Inhalte sind das Stadium der Produktion, also von der Bereitstellung der Rohstoffe bis zum Werkstor der Produktion (cradletogate, Module A1 bis A3), sowie die Errichtung (Module A4 bis 5) und das Ende des Lebensweges (Module C1 bis C4). Darber hinaus erfolgt eine Betrachtung der potenziellen Nutzen und Lasten ber den Lebensweg des Produktes hinaus (Modul D).\n\nModul A\n\nIm Einzelnen werden in Modul A1 die Bereitstellung der Holzrohstoffe sowie die Bereitstellung der Kleb und Zusatzstoffe bilanziert. Hinzu kommen im Wesentlichen die Aufbereitung, Trocknung (inkl. Emissionen), Sortierung und Verpressung der Rohstoffe zu Furnierschichtholz. Die Transporte der stofflich genutzten Rohstoffe, zum Werk werden in Modul A2 bercksichtigt. Modul A3 umfasst die Bereitstellung der Betriebsmittel, der Produktverpackung und des Stroms sowie die Herstellungsprozesse vor Ort. In Modul A4 wird der Transport zur Baustelle bercksichtigt, der im Wesentlichen durch den Vertrieb an Zwischenhndler dargestellt wird. In Modul A5 wird die Entsorgung der Produktverpackung abgebildet, welche den Ausgang des enthaltenen biogenen Kohlenstoffs sowie der enthaltenen Primrenergie (PERM und PENRM) einschliet. Auerdem wird die Verarbeitung der Holzngel auf der Baustelle durch die bliche Druckluftschusstechnik abgebildet. \n\n\nModul B \nModul B wird nicht betrachtet, denn das Verbindungsmittel verbleibt bis zum Lsen der hergestellten Verbindung in den verbundenen (Holz-) Bauteilen und Reste knnen auch nach der Trennung im Holz (-werkstoff) verbleiben, da sie keinen Fremd- oder Strstoff darstellen.\n\nModul C\n\nFr das Modul C1 wird ein manueller Rckbau ohne anfallende Lasten angenommen. Modul C2 bercksichtigt den Transport zum Entsorger und Modul C3 die Aufbereitung und Sortierung des Altholzes. Zudem werden in Modul C3 gem EN 16485 die CO2-quivalente des im Produkt befindlichen holzinhrenten Kohlenstoffs sowie die im Produkt enthaltene erneuerbare und nichterneuerbare Primrenergie (PERM und PENRM) nach normativen Vorgaben berechnet und es weist in C4 keine Abflle zur Deponierung auf. Das ist darin begrndet, dass das Produktsystem am EoL zu Altholz wird, welches gem AltholzV (2020) nicht deponiert werden darf, sondern thermisch oder stofflich verwertet wird. \n\nModul D\n\nModul D bilanziert die thermische Verwertung des Produktes am Ende seines Lebenswegs sowie die daraus resultierenden potenziellen Nutzen und Lasten in Form einer Systemerweiterung.", "lang": "de"}, {"value": "Scope: \nThe nails are intended for use in the production of wood-wood or board-wood connections in load-bearing or stiffening timber structures or timber structures contributing to load-bearing with softwood elements, e.g., solid timber, glue-laminated timber, cross-laminated timber, laminated veneer timber, and similarly glued components, wood-based materials or gypsum fibreboard. \n\nThe declared environmental data relating to 1 kg of LignoLoc® wooden nails is based on a weighted average of Raimund BECK Nageltechnik GmbH wooden nails at the production plant in Mauerkirchen, AT, and has been regionalised for Germany and Austria using generic data. \nSystem boundary: \nThe type of declaration is an EPD Cradle-to-Gate – with options. It comprises the production stage, i.e., from the provision of the raw materials up to the gate of the production factory (cradle-to-gate, modules A1 to A3), construction (modules A4 to 5), and end of life (modules C1 to C4). In addition, potential benefits and burdens are assessed beyond the products life cycle (module D).\n\nModule A\n\nModule A1 assesses the provision of the wood-based raw materials and the provision of the adhesives and additives. In addition, the assessment essentially looks at the processing, drying (incl. emissions), sorting, and pressing of the raw materials into laminated veneer timber. The transport of the materially utilised raw materials to the factory are assessed in module A2. Module A3 covers the provision of the operating materials, product packaging, and electricity as well as the manufacturing processes which take place on location. Module A4 examines the transport to the site of construction, which is essentially reflected by the distribution to intermediate purchasers. Module A5 reflects the disposal of the product packaging, including the outflow of the biogenic carbon content and primary energy content (PERM and PENRM). It also reflects the processing of the wooden nails at the construction site with the usual compressed air tools.\n\nModule B\n\nModule B is not covered because the fastener remains in the connected (wood) components until the connection is separated, and residues may remain in the wood(-based material) after the separation, as they do not constitute foreign or extraneous material.\n\nModule C\n\nManual deconstruction without burdens is assumed for module C1. Module C2 covers the transport to the disposal service, while module C3 covers the processing and sorting of the wood waste. In addition, the CO2 equivalents of the wood-immanent carbon contained in the product and the renewable and non-renewable primary energy (PERM and PENRM) contained in the product are calculated on the basis of normative requirements in module C3 acc. to EN 16485; there is no disposable waste in C4. This is because the product system is turned into wood waste at the end of its life cycle which is not allowed to be disposed under AltholzV (2020), but is subjected to thermal or material utilisation instead. \nModule D Module D assesses the thermal utilisation of the product at the end of its life cycle and the resulting potential benefits and burdens in the form of an expansion of the system.\n\nModul D\n\nModule D assesses the thermal utilisation of the product at the end of its life cycle and the resulting potential benefits and burdens in the form of an expansion of the system.", "lang": "en"}], "other": {"anies": [{"name": "referenceToOriginalEPD", "value": {"shortDescription": {"value": "LIGNOLOC® HOLZNAGEL.pdf", "defaultValue": "LIGNOLOC® HOLZNAGEL.pdf", "lstrings": [{"lang": "de", "value": "LIGNOLOC® HOLZNAGEL.pdf"}]}, "type": "source data set", "uuid": {"uuid": "fdb85628-7396-4df5-af06-b2ecea43d127"}, "refObjectId": "fdb85628-7396-4df5-af06-b2ecea43d127", "resourceURLs": ["https://oekobaudat.de/OEKOBAU.DAT/resource/sources/fdb85628-7396-4df5-af06-b2ecea43d127/LIGNOLOC_HOLZNAGEL_20793.pdf?version=00.01.000"]}}]}}, "validation": {"review": [{"referenceToNameOfReviewerAndInstitution": [{"shortDescription": [{"value": "Institut Bauen und Umwelt e. V.", "lang": "de"}], "type": "contact data set", "refObjectId": "d111dbec-b024-4be5-86c5-752d6eb2cf95", "uri": "../contacts/d111dbec-b024-4be5-86c5-752d6eb2cf95.xml"}], "type": "Accredited third party review"}]}, "complianceDeclarations": {"compliance": [{"referenceToComplianceSystem": {"shortDescription": [{"value": "DIN EN 15804+A2", "lang": "de"}], "type": "source data set", "refObjectId": "c0016b33-8cf7-415c-ac6e-deba0d21440d", "uri": "../sources/c0016b33-8cf7-415c-ac6e-deba0d21440d.xml"}}, {"referenceToComplianceSystem": {"shortDescription": [{"value": "ISO 14025", "lang": "de"}], "type": "source data set", "refObjectId": "4f2eb655-6e44-4874-a95a-e28f5442cd4d", "uri": "../sources/4f2eb655-6e44-4874-a95a-e28f5442cd4d.xml"}}]}}, "administrativeInformation": {"commissionerAndGoal": {"referenceToCommissioner": [{"shortDescription": [{"value": "RAIMUND BECK NAGELTECHNIK GMBH", "lang": "de"}], "type": "contact data set", "refObjectId": "fb0a7618-96df-4e92-94fc-78897260b3d9", "uri": "../contacts/fb0a7618-96df-4e92-94fc-78897260b3d9.xml"}]}, "dataGenerator": {"referenceToPersonOrEntityGeneratingTheDataSet": [{"shortDescription": [{"value": "Thünen-Institut für Holzforschung", "lang": "de"}], "type": "contact data set", "refObjectId": "ddf52906-5279-4989-b886-769f20a62584", "uri": "../contacts/ddf52906-5279-4989-b886-769f20a62584.xml"}]}, "dataEntryBy": {"timeStamp": 1734652800000, "referenceToDataSetFormat": [{"shortDescription": [{"value": "ILCD Format", "lang": "de"}], "type": "source data set", "refObjectId": "a97a0155-0234-4b87-b4ce-a45da52f2a40", "uri": "../sources/a97a0155-0234-4b87-b4ce-a45da52f2a40.xml"}, {"shortDescription": [{"value": "EPD-Datenformaterweiterungen v1.2", "lang": "de"}, {"value": "EPD Data Format Extensions v1.2", "lang": "en"}], "type": "source data set", "refObjectId": "a29449fd-aa2f-4de8-b5d7-4b06b43c6fde", "uri": "../sources/a29449fd-aa2f-4de8-b5d7-4b06b43c6fde.xml"}]}, "publicationAndOwnership": {"dataSetVersion": "00.02.000", "referenceToRegistrationAuthority": {"shortDescription": [{"value": "Institut Bauen und Umwelt e. V.", "lang": "de"}], "type": "contact data set", "refObjectId": "d111dbec-b024-4be5-86c5-752d6eb2cf95", "uri": "../contacts/d111dbec-b024-4be5-86c5-752d6eb2cf95.xml"}, "registrationNumber": "EPD-RAI-20240485-IBA1-DE", "referenceToOwnershipOfDataSet": {"shortDescription": [{"value": "RAIMUND BECK NAGELTECHNIK GMBH", "lang": "de"}], "type": "contact data set", "refObjectId": "fb0a7618-96df-4e92-94fc-78897260b3d9", "uri": "../contacts/fb0a7618-96df-4e92-94fc-78897260b3d9.xml"}, "copyright": true, "licenseType": "Free of charge for all users and uses", "accessRestrictions": [{"value": "None", "lang": "en"}], "other": {"anies": [{"name": "referenceToPublisher", "value": {"shortDescription": [{"value": "Institut Bauen und Umwelt e. V.", "lang": "de"}], "type": "contact data set", "refObjectId": "d111dbec-b024-4be5-86c5-752d6eb2cf95", "uri": "../contacts/d111dbec-b024-4be5-86c5-752d6eb2cf95.xml"}}]}}}, "exchanges": {"exchange": [{"dataSetInternalID": 0, "referenceToFlowDataSet": {"shortDescription": [{"value": "LIGNOLOC® HOLZNAGEL (LIGNOLOC® HOLZNAGEL)", "lang": "de"}], "type": "flow data set", "refObjectId": "6deccde1-3400-b2b9-7473-41193d68b6a2", "uri": "../flows/6deccde1-3400-b2b9-7473-41193d68b6a2.xml"}, "meanAmount": 1.0, "referencesToDataSource": {}, "referenceFlow": true, "resolvedFlowVersion": "00.02.000", "resultingflowAmount": 1.0, "flowProperties": [{"name": [{"lang": "en", "value": "Mass"}, {"lang": "de", "value": "Masse"}], "uuid": "93a60a56-a3c8-11da-a746-0800200b9a66", "referenceFlowProperty": true, "meanValue": 1.0, "referenceUnit": "kg", "unitGroupUUID": "ad38d542-3fe9-439d-9b95-2f5f7752acaf"}], "materialProperties": [{"name": "gross density", "value": "1300.0", "unit": "kg/m^3", "unitDescription": "kilograms per cubic metre"}], "typeOfFlow": "Product flow", "classification": {"classHierarchy": "Holz / Holzwerkstoffe / Elemente aus Holzwerkstoffen", "name": "OEKOBAU.DAT"}}, {"dataSetInternalID": 1, "referenceToFlowDataSet": {"shortDescription": [{"value": "Erneuerbare Primärenergie als Energieträger (PERE)", "lang": "de"}, {"value": "Renewable primary energy as energy carrier (PERE)", "lang": "en"}], "type": "flow data set", "refObjectId": "20f32be5-0398-4288-9b6d-accddd195317", "uri": "../flows/20f32be5-0398-4288-9b6d-accddd195317.xml"}, "exchange direction": "INPUT", "other": {"anies": [{"name": "referenceToUnitGroupDataSet", "value": {"shortDescription": [{"value": "MJ", "lang": "de"}], "type": "unit group data set", "refObjectId": "93a60a57-a3c8-11da-a746-0800200c9a66", "uri": "../unitgroups/93a60a57-a3c8-11da-a746-0800200c9a66.xml"}}, {"value": "11.405085733877", "module": "A1"}, {"value": "0.121901509111535", "module": "A2"}, {"value": "0.228959246162818", "module": "A3"}, {"value": "0.0314674017855694", "module": "A4"}, {"value": "0", "module": "A5"}, {"value": "0", "module": "C1"}, {"value": "3.88961073074839E-06", "module": "C2"}, {"value": "0.000273805852545737", "module": "C3"}, {"value": "0", "module": "C4"}, {"value": "13.1879767124388", "module": "D"}]}, "resolvedFlowVersion": "38.00.000", "flowProperties": [], "typeOfFlow": "Other flow", "classification": {"classHierarchy": "Quantities", "name": "GaBiCategories"}}, {"dataSetInternalID": 2, "referenceToFlowDataSet": {"shortDescription": [{"value": "Erneuerbare Primärenergie zur stofflichen Nutzung (PERM)", "lang": "de"}, {"value": "Renewable primary energy resources as material utilization (PERM)", "lang": "en"}], "type": "flow data set", "refObjectId": "fb3ec0de-548d-4508-aea5-00b73bf6f702", "uri": "../flows/fb3ec0de-548d-4508-aea5-00b73bf6f702.xml"}, "exchange direction": "INPUT", "other": {"anies": [{"name": "referenceToUnitGroupDataSet", "value": {"shortDescription": [{"value": "MJ", "lang": "de"}], "type": "unit group data set", "refObjectId": "93a60a57-a3c8-11da-a746-0800200c9a66", "uri": "../unitgroups/93a60a57-a3c8-11da-a746-0800200c9a66.xml"}}, {"value": "13.200635", "module": "A1"}, {"value": "0", "module": "A2"}, {"value": "0.3198986", "module": "A3"}, {"value": "0", "module": "A4"}, {"value": "-0.3198986", "module": "A5"}, {"value": "0", "module": "C1"}, {"value": "0", "module": "C2"}, {"value": "-13.200635", "module": "C3"}, {"value": "0", "module": "C4"}, {"value": "0", "module": "D"}]}, "resolvedFlowVersion": "38.00.000", "flowProperties": [], "typeOfFlow": "Other flow", "classification": {"classHierarchy": "Quantities", "name": "GaBiCategories"}}, {"dataSetInternalID": 3, "referenceToFlowDataSet": {"shortDescription": [{"value": "Total erneuerbare Primärenergie (PERT)", "lang": "de"}, {"value": "Total use of renewable primary energy resources (PERT)", "lang": "en"}], "type": "flow data set", "refObjectId": "53f97275-fa8a-4cdd-9024-65936002acd0", "uri": "../flows/53f97275-fa8a-4cdd-9024-65936002acd0.xml"}, "exchange direction": "INPUT", "other": {"anies": [{"name": "referenceToUnitGroupDataSet", "value": {"shortDescription": [{"value": "MJ", "lang": "de"}], "type": "unit group data set", "refObjectId": "93a60a57-a3c8-11da-a746-0800200c9a66", "uri": "../unitgroups/93a60a57-a3c8-11da-a746-0800200c9a66.xml"}}, {"value": "24.605720733877", "module": "A1"}, {"value": "0.121901509111535", "module": "A2"}, {"value": "0.548857846162818", "module": "A3"}, {"value": "0.0314674017855694", "module": "A4"}, {"value": "-0.3198986", "module": "A5"}, {"value": "0", "module": "C1"}, {"value": "3.88961073074839E-06", "module": "C2"}, {"value": "-13.2003611941475", "module": "C3"}, {"value": "0", "module": "C4"}, {"value": "13.1879767124388", "module": "D"}]}, "resolvedFlowVersion": "38.00.000", "flowProperties": [], "typeOfFlow": "Other flow", "classification": {"classHierarchy": "Quantities / Environmental quantities / EPD EN 15804 / LCI indicators", "name": "GaBiCategories"}}, {"dataSetInternalID": 4, "referenceToFlowDataSet": {"shortDescription": [{"value": "Nicht-erneuerbare Primärenergie als Energieträger (PENRE)", "lang": "de"}, {"value": "Non renewable primary energy as energy carrier (PENRE)", "lang": "en"}], "type": "flow data set", "refObjectId": "ac857178-2b45-46ec-892a-a9a4332f0372", "uri": "../flows/ac857178-2b45-46ec-892a-a9a4332f0372.xml"}, "exchange direction": "INPUT", "other": {"anies": [{"name": "referenceToUnitGroupDataSet", "value": {"shortDescription": [{"value": "MJ", "lang": "de"}], "type": "unit group data set", "refObjectId": "93a60a57-a3c8-11da-a746-0800200c9a66", "uri": "../unitgroups/93a60a57-a3c8-11da-a746-0800200c9a66.xml"}}, {"value": "22.7801903242471", "module": "A1"}, {"value": "1.72685453940132", "module": "A2"}, {"value": "3.78983566993667", "module": "A3"}, {"value": "0.486922301708445", "module": "A4"}, {"value": "0", "module": "A5"}, {"value": "0", "module": "C1"}, {"value": "5.51001541806292E-05", "module": "C2"}, {"value": "0.000291073214093943", "module": "C3"}, {"value": "0", "module": "C4"}, {"value": "6.82514312263555", "module": "D"}]}, "resolvedFlowVersion": "38.00.000", "flowProperties": [], "typeOfFlow": "Other flow", "classification": {"classHierarchy": "Quantities", "name": "GaBiCategories"}}, {"dataSetInternalID": 5, "referenceToFlowDataSet": {"shortDescription": [{"value": "Nicht-erneuerbare Primärenergie zur stofflichen Nutzung (PENRM)", "lang": "de"}, {"value": "Non renewable primary energy as material utilization (PENRM)", "lang": "en"}], "type": "flow data set", "refObjectId": "1421caa0-679d-4bf4-b282-0eb850ccae27", "uri": "../flows/1421caa0-679d-4bf4-b282-0eb850ccae27.xml"}, "exchange direction": "INPUT", "other": {"anies": [{"name": "referenceToUnitGroupDataSet", "value": {"shortDescription": [{"value": "MJ", "lang": "de"}], "type": "unit group data set", "refObjectId": "93a60a57-a3c8-11da-a746-0800200c9a66", "uri": "../unitgroups/93a60a57-a3c8-11da-a746-0800200c9a66.xml"}}, {"value": "6.85551032240959", "module": "A1"}, {"value": "0", "module": "A2"}, {"value": "2.52", "module": "A3"}, {"value": "0", "module": "A4"}, {"value": "-2.52", "module": "A5"}, {"value": "0", "module": "C1"}, {"value": "0", "module": "C2"}, {"value": "-6.85551032240959", "module": "C3"}, {"value": "0", "module": "C4"}, {"value": "0", "module": "D"}]}, "resolvedFlowVersion": "38.00.000", "flowProperties": [], "typeOfFlow": "Other flow", "classification": {"classHierarchy": "Quantities", "name": "GaBiCategories"}}, {"dataSetInternalID": 6, "referenceToFlowDataSet": {"shortDescription": [{"value": "Total nicht erneuerbare Primärenergie (PENRT)", "lang": "de"}, {"value": "Total use of non renewable primary energy resources (PENRT)", "lang": "en"}], "type": "flow data set", "refObjectId": "06159210-646b-4c8d-8583-da9b3b95a6c1", "uri": "../flows/06159210-646b-4c8d-8583-da9b3b95a6c1.xml"}, "exchange direction": "INPUT", "other": {"anies": [{"name": "referenceToUnitGroupDataSet", "value": {"shortDescription": [{"value": "MJ", "lang": "de"}], "type": "unit group data set", "refObjectId": "93a60a57-a3c8-11da-a746-0800200c9a66", "uri": "../unitgroups/93a60a57-a3c8-11da-a746-0800200c9a66.xml"}}, {"value": "29.6357006466567", "module": "A1"}, {"value": "1.72685453940132", "module": "A2"}, {"value": "6.30983566993667", "module": "A3"}, {"value": "0.486922301708445", "module": "A4"}, {"value": "-2.52", "module": "A5"}, {"value": "0", "module": "C1"}, {"value": "5.51001541806292E-05", "module": "C2"}, {"value": "-6.85521924919549", "module": "C3"}, {"value": "0", "module": "C4"}, {"value": "6.82514312263555", "module": "D"}]}, "resolvedFlowVersion": "38.00.000", "flowProperties": [], "typeOfFlow": "Other flow", "classification": {"classHierarchy": "Quantities / Environmental quantities / EPD EN 15804 / LCI indicators", "name": "GaBiCategories"}}, {"dataSetInternalID": 7, "referenceToFlowDataSet": {"shortDescription": [{"value": "Einsatz von Sekundärstoffen (SM)", "lang": "de"}, {"value": "Use of secondary material (SM)", "lang": "en"}], "type": "flow data set", "refObjectId": "c6a1f35f-2d09-4f54-8dfb-97e502e1ce92", "uri": "../flows/c6a1f35f-2d09-4f54-8dfb-97e502e1ce92.xml"}, "exchange direction": "INPUT", "other": {"anies": [{"name": "referenceToUnitGroupDataSet", "value": {"shortDescription": [{"value": "kg", "lang": "de"}], "type": "unit group data set", "refObjectId": "ad38d542-3fe9-439d-9b95-2f5f7752acaf", "uri": "../unitgroups/ad38d542-3fe9-439d-9b95-2f5f7752acaf.xml"}}, {"value": "0", "module": "A1"}, {"value": "0", "module": "A2"}, {"value": "0", "module": "A3"}, {"value": "0", "module": "A4"}, {"value": "0", "module": "A5"}, {"value": "0", "module": "C1"}, {"value": "0", "module": "C2"}, {"value": "0", "module": "C3"}, {"value": "0", "module": "C4"}, {"value": "0", "module": "D"}]}, "resolvedFlowVersion": "38.00.000", "flowProperties": [], "typeOfFlow": "Other flow", "classification": {"classHierarchy": "Quantities / Environmental quantities / EPD EN 15804 / LCI indicators", "name": "GaBiCategories"}}, {"dataSetInternalID": 8, "referenceToFlowDataSet": {"shortDescription": [{"value": "Erneuerbare Sekundärbrennstoffe (RSF)", "lang": "de"}, {"value": "Use of renewable secondary fuels (RSF)", "lang": "en"}], "type": "flow data set", "refObjectId": "64333088-a55f-4aa2-9a31-c10b07816787", "uri": "../flows/64333088-a55f-4aa2-9a31-c10b07816787.xml"}, "exchange direction": "INPUT", "other": {"anies": [{"name": "referenceToUnitGroupDataSet", "value": {"shortDescription": [{"value": "MJ", "lang": "de"}], "type": "unit group data set", "refObjectId": "93a60a57-a3c8-11da-a746-0800200c9a66", "uri": "../unitgroups/93a60a57-a3c8-11da-a746-0800200c9a66.xml"}}, {"value": "0", "module": "A1"}, {"value": "0", "module": "A2"}, {"value": "0", "module": "A3"}, {"value": "0", "module": "A4"}, {"value": "0", "module": "A5"}, {"value": "0", "module": "C1"}, {"value": "0", "module": "C2"}, {"value": "0", "module": "C3"}, {"value": "0", "module": "C4"}, {"value": "13.200635", "module": "D"}]}, "resolvedFlowVersion": "38.00.000", "flowProperties": [], "typeOfFlow": "Other flow", "classification": {"classHierarchy": "Quantities / Environmental quantities / EPD EN 15804 / LCI indicators", "name": "GaBiCategories"}}, {"dataSetInternalID": 9, "referenceToFlowDataSet": {"shortDescription": [{"value": "Nicht erneuerbare Sekundärbrennstoffe (NRSF)", "lang": "de"}, {"value": "Use of non renewable secondary fuels (NRSF)", "lang": "en"}], "type": "flow data set", "refObjectId": "89def144-d39a-4287-b86f-efde453ddcb2", "uri": "../flows/89def144-d39a-4287-b86f-efde453ddcb2.xml"}, "exchange direction": "INPUT", "other": {"anies": [{"name": "referenceToUnitGroupDataSet", "value": {"shortDescription": [{"value": "MJ", "lang": "de"}], "type": "unit group data set", "refObjectId": "93a60a57-a3c8-11da-a746-0800200c9a66", "uri": "../unitgroups/93a60a57-a3c8-11da-a746-0800200c9a66.xml"}}, {"value": "0", "module": "A1"}, {"value": "0", "module": "A2"}, {"value": "0", "module": "A3"}, {"value": "0", "module": "A4"}, {"value": "0", "module": "A5"}, {"value": "0", "module": "C1"}, {"value": "0", "module": "C2"}, {"value": "0", "module": "C3"}, {"value": "0", "module": "C4"}, {"value": "6.85551032240959", "module": "D"}]}, "resolvedFlowVersion": "38.00.000", "flowProperties": [], "typeOfFlow": "Other flow", "classification": {"classHierarchy": "Quantities / Environmental quantities / EPD EN 15804 / LCI indicators", "name": "GaBiCategories"}}, {"dataSetInternalID": 10, "referenceToFlowDataSet": {"shortDescription": [{"value": "Einsatz von Süßwasserressourcen (FW)", "lang": "de"}, {"value": "Use of net fresh water (FW)", "lang": "en"}], "type": "flow data set", "refObjectId": "3cf952c8-f3a4-461d-8c96-96456ca62246", "uri": "../flows/3cf952c8-f3a4-461d-8c96-96456ca62246.xml"}, "exchange direction": "INPUT", "other": {"anies": [{"name": "referenceToUnitGroupDataSet", "value": {"shortDescription": [{"value": "m^3", "lang": "de"}], "type": "unit group data set", "refObjectId": "cd950537-0a98-4044-9ba7-9f9a68d0a504", "uri": "../unitgroups/cd950537-0a98-4044-9ba7-9f9a68d0a504.xml"}}, {"value": "0.00404878073689541", "module": "A1"}, {"value": "0.000134331507383379", "module": "A2"}, {"value": "0.000732745597991614", "module": "A3"}, {"value": "0", "module": "A4"}, {"value": "0", "module": "A5"}, {"value": "0", "module": "C1"}, {"value": "4.28622480889802E-09", "module": "C2"}, {"value": "9.59570002064078E-08", "module": "C3"}, {"value": "0", "module": "C4"}, {"value": "8.75220972261901E-06", "module": "D"}]}, "resolvedFlowVersion": "38.00.000", "flowProperties": [], "typeOfFlow": "Other flow", "classification": {"classHierarchy": "Quantities / Environmental quantities / EPD EN 15804 / LCI indicators", "name": "GaBiCategories"}}, {"dataSetInternalID": 11, "referenceToFlowDataSet": {"shortDescription": [{"value": "Gefährlicher Abfall zur Deponie (HWD)", "lang": "de"}, {"value": "Hazardous waste disposed (HWD)", "lang": "en"}], "type": "flow data set", "refObjectId": "430f9e0f-59b2-46a0-8e0d-55e0e84948fc", "uri": "../flows/430f9e0f-59b2-46a0-8e0d-55e0e84948fc.xml"}, "exchange direction": "OUTPUT", "other": {"anies": [{"name": "referenceToUnitGroupDataSet", "value": {"shortDescription": [{"value": "kg", "lang": "de"}], "type": "unit group data set", "refObjectId": "ad38d542-3fe9-439d-9b95-2f5f7752acaf", "uri": "../unitgroups/ad38d542-3fe9-439d-9b95-2f5f7752acaf.xml"}}, {"value": "0.00134707723094369", "module": "A1"}, {"value": "0.000999898652718618", "module": "A2"}, {"value": "2.23273137704155E-06", "module": "A3"}, {"value": "0", "module": "A4"}, {"value": "0.000345718613318775", "module": "A5"}, {"value": "0", "module": "C1"}, {"value": "-1.37411269284097E-06", "module": "C2"}, {"value": "0", "module": "C3"}, {"value": "0", "module": "C4"}, {"value": "2.8464874046542E-08", "module": "D"}]}, "resolvedFlowVersion": "38.00.000", "flowProperties": [], "typeOfFlow": "Other flow", "classification": {"classHierarchy": "Quantities / Environmental quantities / EPD EN 15804 / LCI indicators", "name": "GaBiCategories"}}, {"dataSetInternalID": 12, "referenceToFlowDataSet": {"shortDescription": [{"value": "Entsorgter nicht gefährlicher Abfall (NHWD)", "lang": "de"}, {"value": "Non hazardous waste disposed (NHWD)", "lang": "en"}], "type": "flow data set", "refObjectId": "b29ef66b-e286-4afa-949f-62f1a7b4d7fa", "uri": "../flows/b29ef66b-e286-4afa-949f-62f1a7b4d7fa.xml"}, "exchange direction": "OUTPUT", "other": {"anies": [{"name": "referenceToUnitGroupDataSet", "value": {"shortDescription": [{"value": "kg", "lang": "de"}], "type": "unit group data set", "refObjectId": "ad38d542-3fe9-439d-9b95-2f5f7752acaf", "uri": "../unitgroups/ad38d542-3fe9-439d-9b95-2f5f7752acaf.xml"}}, {"value": "0.021703117969308", "module": "A1"}, {"value": "0.0175398508116245", "module": "A2"}, {"value": "0.000248883295392099", "module": "A3"}, {"value": "0", "module": "A4"}, {"value": "0.0036214216621491", "module": "A5"}, {"value": "0", "module": "C1"}, {"value": "-1.80074601353489E-05", "module": "C2"}, {"value": "0", "module": "C3"}, {"value": "0", "module": "C4"}, {"value": "2.74921803062404E-07", "module": "D"}]}, "resolvedFlowVersion": "38.00.000", "flowProperties": [], "typeOfFlow": "Other flow", "classification": {"classHierarchy": "Quantities / Environmental quantities / EPD EN 15804 / LCI indicators", "name": "GaBiCategories"}}, {"dataSetInternalID": 13, "referenceToFlowDataSet": {"shortDescription": [{"value": "Entsorgter radioaktiver Abfall (RWD)", "lang": "de"}, {"value": "Radioactive waste disposed (RWD)", "lang": "en"}], "type": "flow data set", "refObjectId": "3449546e-52ad-4b39-b809-9fb77cea8ff6", "uri": "../flows/3449546e-52ad-4b39-b809-9fb77cea8ff6.xml"}, "exchange direction": "OUTPUT", "other": {"anies": [{"name": "referenceToUnitGroupDataSet", "value": {"shortDescription": [{"value": "kg", "lang": "de"}], "type": "unit group data set", "refObjectId": "ad38d542-3fe9-439d-9b95-2f5f7752acaf", "uri": "../unitgroups/ad38d542-3fe9-439d-9b95-2f5f7752acaf.xml"}}, {"value": "1.80805228368205E-09", "module": "A1"}, {"value": "1.16205004877465E-09", "module": "A2"}, {"value": "6.3895643348591E-12", "module": "A3"}, {"value": "0", "module": "A4"}, {"value": "6.39902195632484E-10", "module": "A5"}, {"value": "0", "module": "C1"}, {"value": "-1.52508215669768E-12", "module": "C2"}, {"value": "0", "module": "C3"}, {"value": "0", "module": "C4"}, {"value": "-5.66747697524116E-14", "module": "D"}]}, "resolvedFlowVersion": "38.00.000", "flowProperties": [], "typeOfFlow": "Other flow", "classification": {"classHierarchy": "Quantities / Environmental quantities / EPD EN 15804 / LCI indicators", "name": "GaBiCategories"}}, {"dataSetInternalID": 14, "referenceToFlowDataSet": {"shortDescription": [{"value": "Komponenten für die Wiederverwendung (CRU)", "lang": "de"}, {"value": "Components for re-use (CRU)", "lang": "en"}], "type": "flow data set", "refObjectId": "a2b32f97-3fc7-4af2-b209-525bc6426f33", "uri": "../flows/a2b32f97-3fc7-4af2-b209-525bc6426f33.xml"}, "exchange direction": "OUTPUT", "other": {"anies": [{"name": "referenceToUnitGroupDataSet", "value": {"shortDescription": [{"value": "kg", "lang": "de"}], "type": "unit group data set", "refObjectId": "ad38d542-3fe9-439d-9b95-2f5f7752acaf", "uri": "../unitgroups/ad38d542-3fe9-439d-9b95-2f5f7752acaf.xml"}}, {"value": "0", "module": "A1"}, {"value": "0", "module": "A2"}, {"value": "0", "module": "A3"}, {"value": "0", "module": "A4"}, {"value": "0", "module": "A5"}, {"value": "0", "module": "C1"}, {"value": "0", "module": "C2"}, {"value": "0", "module": "C3"}, {"value": "0", "module": "C4"}, {"value": "0", "module": "D"}]}, "resolvedFlowVersion": "38.00.000", "flowProperties": [], "typeOfFlow": "Other flow", "classification": {"classHierarchy": "Quantities / Environmental quantities / EPD EN 15804 / LCI indicators", "name": "GaBiCategories"}}, {"dataSetInternalID": 15, "referenceToFlowDataSet": {"shortDescription": [{"value": "Stoffe zum Recycling (MFR)", "lang": "de"}, {"value": "Materials for recycling (MFR)", "lang": "en"}], "type": "flow data set", "refObjectId": "d7fe48a5-4103-49c8-9aae-b0b5dfdbd6ae", "uri": "../flows/d7fe48a5-4103-49c8-9aae-b0b5dfdbd6ae.xml"}, "exchange direction": "OUTPUT", "other": {"anies": [{"name": "referenceToUnitGroupDataSet", "value": {"shortDescription": [{"value": "kg", "lang": "de"}], "type": "unit group data set", "refObjectId": "ad38d542-3fe9-439d-9b95-2f5f7752acaf", "uri": "../unitgroups/ad38d542-3fe9-439d-9b95-2f5f7752acaf.xml"}}, {"value": "0", "module": "A1"}, {"value": "0", "module": "A2"}, {"value": "0", "module": "A3"}, {"value": "0", "module": "A4"}, {"value": "0", "module": "A5"}, {"value": "0", "module": "C1"}, {"value": "0", "module": "C2"}, {"value": "0", "module": "C3"}, {"value": "0", "module": "C4"}, {"value": "0", "module": "D"}]}, "resolvedFlowVersion": "38.00.000", "flowProperties": [], "typeOfFlow": "Other flow", "classification": {"classHierarchy": "Quantities / Environmental quantities / EPD EN 15804 / LCI indicators", "name": "GaBiCategories"}}, {"dataSetInternalID": 16, "referenceToFlowDataSet": {"shortDescription": [{"value": "Stoffe für die Energierückgewinnung (MER)", "lang": "de"}, {"value": "Materials for energy recovery (MER)", "lang": "en"}], "type": "flow data set", "refObjectId": "59a9181c-3aaf-46ee-8b13-2b3723b6e447", "uri": "../flows/59a9181c-3aaf-46ee-8b13-2b3723b6e447.xml"}, "exchange direction": "OUTPUT", "other": {"anies": [{"name": "referenceToUnitGroupDataSet", "value": {"shortDescription": [{"value": "kg", "lang": "de"}], "type": "unit group data set", "refObjectId": "ad38d542-3fe9-439d-9b95-2f5f7752acaf", "uri": "../unitgroups/ad38d542-3fe9-439d-9b95-2f5f7752acaf.xml"}}, {"value": "0", "module": "A1"}, {"value": "0", "module": "A2"}, {"value": "1.89189189189189", "module": "A3"}, {"value": "0", "module": "A4"}, {"value": "0.0166", "module": "A5"}, {"value": "0", "module": "C1"}, {"value": "0", "module": "C2"}, {"value": "1", "module": "C3"}, {"value": "0", "module": "C4"}, {"value": "0", "module": "D"}]}, "resolvedFlowVersion": "38.00.000", "flowProperties": [], "typeOfFlow": "Other flow", "classification": {"classHierarchy": "Quantities / Environmental quantities / EPD EN 15804 / LCI indicators", "name": "GaBiCategories"}}, {"dataSetInternalID": 17, "referenceToFlowDataSet": {"shortDescription": [{"value": "Exportierte elektrische Energie (EEE)", "lang": "de"}, {"value": "Exported electrical energy (EEE)", "lang": "en"}], "type": "flow data set", "refObjectId": "4da0c987-2b76-40d6-9e9e-82a017aaaf29", "uri": "../flows/4da0c987-2b76-40d6-9e9e-82a017aaaf29.xml"}, "exchange direction": "OUTPUT", "other": {"anies": [{"name": "referenceToUnitGroupDataSet", "value": {"shortDescription": [{"value": "MJ", "lang": "de"}], "type": "unit group data set", "refObjectId": "93a60a57-a3c8-11da-a746-0800200c9a66", "uri": "../unitgroups/93a60a57-a3c8-11da-a746-0800200c9a66.xml"}}, {"value": "0", "module": "A1"}, {"value": "0", "module": "A2"}, {"value": "0.0198429549503517", "module": "A3"}, {"value": "0", "module": "A4"}, {"value": "0", "module": "A5"}, {"value": "0", "module": "C1"}, {"value": "0", "module": "C2"}, {"value": "0", "module": "C3"}, {"value": "0", "module": "C4"}, {"value": "0", "module": "D"}]}, "resolvedFlowVersion": "38.00.000", "flowProperties": [], "typeOfFlow": "Other flow", "classification": {"classHierarchy": "Quantities / Environmental quantities / EPD EN 15804 / LCI indicators", "name": "GaBiCategories"}}, {"dataSetInternalID": 18, "referenceToFlowDataSet": {"shortDescription": [{"value": "Exportierte thermische Energie (EET)", "lang": "de"}, {"value": "Exported thermal energy (EET)", "lang": "en"}], "type": "flow data set", "refObjectId": "98daf38a-7a79-46d3-9a37-2b7bd0955810", "uri": "../flows/98daf38a-7a79-46d3-9a37-2b7bd0955810.xml"}, "exchange direction": "OUTPUT", "other": {"anies": [{"name": "referenceToUnitGroupDataSet", "value": {"shortDescription": [{"value": "MJ", "lang": "de"}], "type": "unit group data set", "refObjectId": "93a60a57-a3c8-11da-a746-0800200c9a66", "uri": "../unitgroups/93a60a57-a3c8-11da-a746-0800200c9a66.xml"}}, {"value": "0", "module": "A1"}, {"value": "0", "module": "A2"}, {"value": "0.0359726535259619", "module": "A3"}, {"value": "0", "module": "A4"}, {"value": "0", "module": "A5"}, {"value": "0", "module": "C1"}, {"value": "0", "module": "C2"}, {"value": "0", "module": "C3"}, {"value": "0", "module": "C4"}, {"value": "0", "module": "D"}]}, "resolvedFlowVersion": "38.00.000", "flowProperties": [], "typeOfFlow": "Other flow", "classification": {"classHierarchy": "Quantities / Environmental quantities / EPD EN 15804 / LCI indicators", "name": "GaBiCategories"}}]}, "LCIAResults": {"LCIAResult": [{"referenceToLCIAMethodDataSet": {"shortDescription": [{"value": "Globales Erwärmungspotenzial total (GWP-total)", "lang": "de"}, {"value": "Global Warming Potential total (GWP-total)", "lang": "en"}], "type": "LCIA method data set", "refObjectId": "6a37f984-a4b3-458a-a20a-64418c145fa2", "uri": "../lciamethods/6a37f984-a4b3-458a-a20a-64418c145fa2.xml"}, "other": {"anies": [{"name": "referenceToUnitGroupDataSet", "value": {"shortDescription": [{"value": "kg CO_(2)-Äq.", "lang": "de"}], "type": "unit group data set", "refObjectId": "1ebf3012-d0db-4de2-aefd-ef30cedb0be1", "uri": "../unitgroups/1ebf3012-d0db-4de2-aefd-ef30cedb0be1.xml"}}, {"value": "-0.113298152426804", "module": "A1"}, {"value": "0.124434854188881", "module": "A2"}, {"value": "0.221976663975788", "module": "A3"}, {"value": "0.0354473521477065", "module": "A4"}, {"value": "0.0424333333333333", "module": "A5"}, {"value": "0", "module": "C1"}, {"value": "2.05737386798985E-05", "module": "C2"}, {"value": "1.2558336207078", "module": "C3"}, {"value": "0", "module": "C4"}, {"value": "0.00014151950038588", "module": "D"}]}}, {"referenceToLCIAMethodDataSet": {"shortDescription": [{"value": "Globales Erwärmungspotenzial fossil (GWP-fossil)", "lang": "de"}, {"value": "Global Warming Potential fossil fuels (GWP-fossil)", "lang": "en"}], "type": "LCIA method data set", "refObjectId": "5f635281-343e-44fb-83df-1971b155e6b6", "uri": "../lciamethods/5f635281-343e-44fb-83df-1971b155e6b6.xml"}, "other": {"anies": [{"name": "referenceToUnitGroupDataSet", "value": {"shortDescription": [{"value": "kg CO_(2)-Äq.", "lang": "de"}], "type": "unit group data set", "refObjectId": "1ebf3012-d0db-4de2-aefd-ef30cedb0be1", "uri": "../unitgroups/1ebf3012-d0db-4de2-aefd-ef30cedb0be1.xml"}}, {"value": "1.13956051117284", "module": "A1"}, {"value": "0.124042855902026", "module": "A2"}, {"value": "0.263600761134397", "module": "A3"}, {"value": "0.0356087237145945", "module": "A4"}, {"value": "0", "module": "A5"}, {"value": "0", "module": "C1"}, {"value": "2.0561230871307E-05", "module": "C2"}, {"value": "0", "module": "C3"}, {"value": "0", "module": "C4"}, {"value": "0.00014151950038588", "module": "D"}]}}, {"referenceToLCIAMethodDataSet": {"shortDescription": [{"value": "Globales Erwärmungspotenzial biogen (GWP-biogenic)", "lang": "de"}, {"value": "Global Warming Potential biogenic (GWP-biogenic)", "lang": "en"}], "type": "LCIA method data set", "refObjectId": "2356e1ab-0185-4db5-86e5-16de51c7485c", "uri": "../lciamethods/2356e1ab-0185-4db5-86e5-16de51c7485c.xml"}, "other": {"anies": [{"name": "referenceToUnitGroupDataSet", "value": {"shortDescription": [{"value": "kg CO_(2)-Äq.", "lang": "de"}], "type": "unit group data set", "refObjectId": "1ebf3012-d0db-4de2-aefd-ef30cedb0be1", "uri": "../unitgroups/1ebf3012-d0db-4de2-aefd-ef30cedb0be1.xml"}}, {"value": "-1.25285866359964", "module": "A1"}, {"value": "0.000391998286855159", "module": "A2"}, {"value": "-0.0416240971586086", "module": "A3"}, {"value": "-0.000161371566887962", "module": "A4"}, {"value": "0.0424333333333333", "module": "A5"}, {"value": "0", "module": "C1"}, {"value": "1.25078085915389E-08", "module": "C2"}, {"value": "1.2558336207078", "module": "C3"}, {"value": "0", "module": "C4"}, {"value": "0", "module": "D"}]}}, {"referenceToLCIAMethodDataSet": {"shortDescription": [{"value": "Globales Erwärmungspotenzial luluc (GWP-luluc)", "lang": "de"}, {"value": "Global Warming Potential luluc (GWP-luluc)", "lang": "en"}], "type": "LCIA method data set", "refObjectId": "4331bbdb-978a-490d-8707-eeb047f01a55", "uri": "../lciamethods/4331bbdb-978a-490d-8707-eeb047f01a55.xml"}, "other": {"anies": [{"name": "referenceToUnitGroupDataSet", "value": {"shortDescription": [{"value": "kg CO_(2)-Äq.", "lang": "de"}], "type": "unit group data set", "refObjectId": "1ebf3012-d0db-4de2-aefd-ef30cedb0be1", "uri": "../unitgroups/1ebf3012-d0db-4de2-aefd-ef30cedb0be1.xml"}}, {"module": "A1"}, {"module": "A2"}, {"module": "A3"}, {"module": "A4"}, {"module": "A5"}, {"module": "C1"}, {"module": "C2"}, {"module": "C3"}, {"module": "C4"}, {"module": "D"}]}}, {"referenceToLCIAMethodDataSet": {"shortDescription": [{"value": "Abbau Potential der stratosphärischen Ozonschicht (ODP)", "lang": "de"}, {"value": "Depletion potential of the stratospheric ozone layer (ODP)", "lang": "en"}], "type": "LCIA method data set", "refObjectId": "b5c629d6-def3-11e6-bf01-fe55135034f3", "uri": "../lciamethods/b5c629d6-def3-11e6-bf01-fe55135034f3.xml"}, "other": {"anies": [{"name": "referenceToUnitGroupDataSet", "value": {"shortDescription": [{"value": "kg CFC11-Äq.", "lang": "de"}], "type": "unit group data set", "refObjectId": "d9e957c9-7309-4474-bf3a-7777df6c4e5b", "uri": "../unitgroups/d9e957c9-7309-4474-bf3a-7777df6c4e5b.xml"}}, {"value": "5.83294778181726E-12", "module": "A1"}, {"value": "1.1090033472061E-14", "module": "A2"}, {"value": "-2.56882629404945E-15", "module": "A3"}, {"value": "6.2807535700003E-15", "module": "A4"}, {"value": "0", "module": "A5"}, {"value": "0", "module": "C1"}, {"value": "3.53858729983563E-19", "module": "C2"}, {"value": "5.648833858802E-16", "module": "C3"}, {"value": "0", "module": "C4"}, {"value": "-2.60496439244255E-14", "module": "D"}]}}, {"referenceToLCIAMethodDataSet": {"shortDescription": [{"value": "Versauerungspotenzial von Boden und Wasser (AP)", "lang": "de"}, {"value": "Acidification potential of land and water (AP)", "lang": "en"}], "type": "LCIA method data set", "refObjectId": "b5c611c6-def3-11e6-bf01-fe55135034f3", "uri": "../lciamethods/b5c611c6-def3-11e6-bf01-fe55135034f3.xml"}, "other": {"anies": [{"name": "referenceToUnitGroupDataSet", "value": {"shortDescription": [{"value": "mol H^(+)-Äq.", "lang": "de"}], "type": "unit group data set", "refObjectId": "42e089ac-92bf-4bf2-8ca1-5fc40d18f2ed", "uri": "../unitgroups/42e089ac-92bf-4bf2-8ca1-5fc40d18f2ed.xml"}}, {"value": "0.00340832206734403", "module": "A1"}, {"value": "0.000777538578540986", "module": "A2"}, {"value": "0.00032465658563878", "module": "A3"}, {"value": "6.34692881942245E-05", "module": "A4"}, {"value": "0", "module": "A5"}, {"value": "0", "module": "C1"}, {"value": "2.4809556671663E-08", "module": "C2"}, {"value": "3.15552348017441E-08", "module": "C3"}, {"value": "0", "module": "C4"}, {"value": "-1.15271144126913E-06", "module": "D"}]}}, {"referenceToLCIAMethodDataSet": {"shortDescription": [{"value": "Eutrophierungspotenzial Süßwasser (EP-freshwater)", "lang": "de"}, {"value": "Eutrophication potential aquatic freshwater (EP-freshwater)", "lang": "en"}], "type": "LCIA method data set", "refObjectId": "b53ec18f-7377-4ad3-86eb-cc3f4f276b2b", "uri": "../lciamethods/b53ec18f-7377-4ad3-86eb-cc3f4f276b2b.xml"}, "other": {"anies": [{"name": "referenceToUnitGroupDataSet", "value": {"shortDescription": [{"value": "kg P-Äq.", "lang": "de"}], "type": "unit group data set", "refObjectId": "0429039d-a61d-4590-ba67-aa4a20a810a1", "uri": "../unitgroups/0429039d-a61d-4590-ba67-aa4a20a810a1.xml"}}, {"value": "2.06637770501304E-06", "module": "A1"}, {"value": "4.61869587981743E-07", "module": "A2"}, {"value": "2.7969776586531E-08", "module": "A3"}, {"value": "8.36125087665586E-08", "module": "A4"}, {"value": "0", "module": "A5"}, {"value": "0", "module": "C1"}, {"value": "1.47372491014562E-11", "module": "C2"}, {"value": "1.23528655743702E-10", "module": "C3"}, {"value": "0", "module": "C4"}, {"value": "-5.72815858017134E-09", "module": "D"}]}}, {"referenceToLCIAMethodDataSet": {"shortDescription": [{"value": "Eutrophierungspotenzial Salzwasser (EP-marine)", "lang": "de"}, {"value": "Eutrophication potential aquatic marine (EP-marine)", "lang": "en"}], "type": "LCIA method data set", "refObjectId": "b5c619fa-def3-11e6-bf01-fe55135034f3", "uri": "../lciamethods/b5c619fa-def3-11e6-bf01-fe55135034f3.xml"}, "other": {"anies": [{"name": "referenceToUnitGroupDataSet", "value": {"shortDescription": [{"value": "kg N-Äq.", "lang": "de"}], "type": "unit group data set", "refObjectId": "d05bb823-ecdf-4686-8c40-bf1d9257859f", "uri": "../unitgroups/d05bb823-ecdf-4686-8c40-bf1d9257859f.xml"}}, {"value": "0.00130266161756333", "module": "A1"}, {"value": "0.000381234084176863", "module": "A2"}, {"value": "0.000110084270464765", "module": "A3"}, {"value": "2.68336047836658E-05", "module": "A4"}, {"value": "0", "module": "A5"}, {"value": "0", "module": "C1"}, {"value": "1.21643464100565E-08", "module": "C2"}, {"value": "1.03373725320913E-08", "module": "C3"}, {"value": "0", "module": "C4"}, {"value": "-5.30677100203286E-07", "module": "D"}]}}, {"referenceToLCIAMethodDataSet": {"shortDescription": [{"value": "Eutrophierungspotenzial Land (EP-terrestrial)", "lang": "de"}, {"value": "Eutrophication potential terrestrial (EP-terrestrial)", "lang": "en"}], "type": "LCIA method data set", "refObjectId": "b5c614d2-def3-11e6-bf01-fe55135034f3", "uri": "../lciamethods/b5c614d2-def3-11e6-bf01-fe55135034f3.xml"}, "other": {"anies": [{"name": "referenceToUnitGroupDataSet", "value": {"shortDescription": [{"value": "mol N-Äq.", "lang": "de"}], "type": "unit group data set", "refObjectId": "71b4d617-0ec9-4d3f-b65e-e438940c2401", "uri": "../unitgroups/71b4d617-0ec9-4d3f-b65e-e438940c2401.xml"}}, {"value": "0.0151380799813092", "module": "A1"}, {"value": "0.00422708295344352", "module": "A2"}, {"value": "0.00121249778327858", "module": "A3"}, {"value": "0.000305753577965128", "module": "A4"}, {"value": "0", "module": "A5"}, {"value": "0", "module": "C1"}, {"value": "1.34876978433745E-07", "module": "C2"}, {"value": "1.06778098740364E-07", "module": "C3"}, {"value": "0", "module": "C4"}, {"value": "-3.6059750081066E-06", "module": "D"}]}}, {"referenceToLCIAMethodDataSet": {"shortDescription": [{"value": "Bildungspotential für troposphärisches Ozon (POCP)", "lang": "de"}, {"value": "Formation potential of tropospheric ozone photochemical oxidants (POCP)", "lang": "en"}], "type": "LCIA method data set", "refObjectId": "b5c610fe-def3-11e6-bf01-fe55135034f3", "uri": "../lciamethods/b5c610fe-def3-11e6-bf01-fe55135034f3.xml"}, "other": {"anies": [{"name": "referenceToUnitGroupDataSet", "value": {"shortDescription": [{"value": "kg NMVOC-Äq.", "lang": "de"}], "type": "unit group data set", "refObjectId": "d27c25f8-fbc1-44c6-b47b-4adbae4199c6", "uri": "../unitgroups/d27c25f8-fbc1-44c6-b47b-4adbae4199c6.xml"}}, {"value": "0.00373307482143343", "module": "A1"}, {"value": "0.000717366380528403", "module": "A2"}, {"value": "0.000303898451352359", "module": "A3"}, {"value": "5.66120480188377E-05", "module": "A4"}, {"value": "0", "module": "A5"}, {"value": "0", "module": "C1"}, {"value": "2.28895933439874E-08", "module": "C2"}, {"value": "2.47422877813247E-08", "module": "C3"}, {"value": "0", "module": "C4"}, {"value": "-1.32837812429575E-06", "module": "D"}]}}, {"referenceToLCIAMethodDataSet": {"shortDescription": [{"value": "Potenzial für den abiotischen Abbau nicht fossiler Ressourcen (ADPE)", "lang": "de"}, {"value": "Abiotic depletion potential for non fossil resources (ADPE)", "lang": "en"}], "type": "LCIA method data set", "refObjectId": "b2ad6494-c78d-11e6-9d9d-cec0c932ce01", "uri": "../lciamethods/b2ad6494-c78d-11e6-9d9d-cec0c932ce01.xml"}, "other": {"anies": [{"name": "referenceToUnitGroupDataSet", "value": {"shortDescription": [{"value": "kg Sb-Äq.", "lang": "de"}], "type": "unit group data set", "refObjectId": "54ccd2d9-a32a-4fc2-923d-f2c8c93e89d4", "uri": "../unitgroups/54ccd2d9-a32a-4fc2-923d-f2c8c93e89d4.xml"}}, {"value": "5.82444587354322E-08", "module": "A1"}, {"value": "8.22688796232248E-09", "module": "A2"}, {"value": "3.49282059681642E-08", "module": "A3"}, {"value": "2.55363315092304E-09", "module": "A4"}, {"value": "0", "module": "A5"}, {"value": "0", "module": "C1"}, {"value": "2.62502014389635E-13", "module": "C2"}, {"value": "3.75903917595707E-12", "module": "C3"}, {"value": "0", "module": "C4"}, {"value": "-1.83150128323652E-10", "module": "D"}]}}, {"referenceToLCIAMethodDataSet": {"shortDescription": [{"value": "Potenzial für den abiotischen Abbau fossiler Brennstoffe (ADPF)", "lang": "de"}, {"value": "Abiotic depletion potential for fossil resources (ADPF)", "lang": "en"}], "type": "LCIA method data set", "refObjectId": "b2ad6110-c78d-11e6-9d9d-cec0c932ce01", "uri": "../lciamethods/b2ad6110-c78d-11e6-9d9d-cec0c932ce01.xml"}, "other": {"anies": [{"name": "referenceToUnitGroupDataSet", "value": {"shortDescription": [{"value": "MJ", "lang": "de"}], "type": "unit group data set", "refObjectId": "93a60a57-a3c8-11da-a746-0800200c9a66", "uri": "../unitgroups/93a60a57-a3c8-11da-a746-0800200c9a66.xml"}}, {"value": "22.7717261102891", "module": "A1"}, {"value": "1.72242360168573", "module": "A2"}, {"value": "3.78901923264971", "module": "A3"}, {"value": "0.486661179722092", "module": "A4"}, {"value": "0", "module": "A5"}, {"value": "0", "module": "C1"}, {"value": "5.49587726422753E-05", "module": "C2"}, {"value": "0.000290963780286144", "module": "C3"}, {"value": "0", "module": "C4"}, {"value": "-0.0303623401098994", "module": "D"}]}}, {"referenceToLCIAMethodDataSet": {"shortDescription": [{"value": "Wassernutzung (WDP)", "lang": "de"}, {"value": "Water use (WDP)", "lang": "en"}], "type": "LCIA method data set", "refObjectId": "b2ad66ce-c78d-11e6-9d9d-cec0c932ce01", "uri": "../lciamethods/b2ad66ce-c78d-11e6-9d9d-cec0c932ce01.xml"}, "other": {"anies": [{"name": "referenceToUnitGroupDataSet", "value": {"shortDescription": [{"value": "m^(3) Welt-Äq. entzogen", "lang": "de"}], "type": "unit group data set", "refObjectId": "6ae2df01-888e-46c8-b17d-49fa3869b476", "uri": "../unitgroups/6ae2df01-888e-46c8-b17d-49fa3869b476.xml"}}, {"value": "0.0305112444879512", "module": "A1"}, {"value": "0.00145993779639435", "module": "A2"}, {"value": "0.0089896519296755", "module": "A3"}, {"value": "0.000186692369483224", "module": "A4"}, {"value": "0", "module": "A5"}, {"value": "0", "module": "C1"}, {"value": "4.65834242780785E-08", "module": "C2"}, {"value": "5.91429630256781E-07", "module": "C3"}, {"value": "0", "module": "C4"}, {"value": "0.000539113931355792", "module": "D"}]}}, {"referenceToLCIAMethodDataSet": {"shortDescription": [{"value": "Auftreten von Krankheiten aufgrund von Feinstaubemissionen (PM)", "lang": "de"}, {"value": "Incidence of disease due to PM emissions (PM)", "lang": "en"}], "type": "LCIA method data set", "refObjectId": "b5c602c6-def3-11e6-bf01-fe55135034f3", "uri": "../lciamethods/b5c602c6-def3-11e6-bf01-fe55135034f3.xml"}, "other": {"anies": [{"name": "referenceToUnitGroupDataSet", "value": {"shortDescription": [{"value": "Krankheitsfälle", "lang": "de"}], "type": "unit group data set", "refObjectId": "3883559b-648f-4afc-8ba2-0bd24f3affa3", "uri": "../unitgroups/3883559b-648f-4afc-8ba2-0bd24f3affa3.xml"}}, {"value": "2.75294135855769E-08", "module": "A1"}, {"value": "4.56737885459914E-09", "module": "A2"}, {"value": "4.79598042521099E-09", "module": "A3"}, {"value": "3.8834675037873E-10", "module": "A4"}, {"value": "0", "module": "A5"}, {"value": "0", "module": "C1"}, {"value": "1.45735076897101E-13", "module": "C2"}, {"value": "2.48686710569422E-13", "module": "C3"}, {"value": "0", "module": "C4"}, {"value": "-8.27721871107549E-12", "module": "D"}]}}, {"referenceToLCIAMethodDataSet": {"shortDescription": [{"value": "Wirkung durch Exposition des Menschen mit U235 (IR)", "lang": "de"}, {"value": "Human exposure efficiency relative to U235 (IR)", "lang": "en"}], "type": "LCIA method data set", "refObjectId": "b5c632be-def3-11e6-bf01-fe55135034f3", "uri": "../lciamethods/b5c632be-def3-11e6-bf01-fe55135034f3.xml"}, "other": {"anies": [{"name": "referenceToUnitGroupDataSet", "value": {"shortDescription": [{"value": "kBq U235-Äq.", "lang": "de"}], "type": "unit group data set", "refObjectId": "456b05bf-1415-44a9-9993-02452f554c09", "uri": "../unitgroups/456b05bf-1415-44a9-9993-02452f554c09.xml"}}, {"value": "0.0861090432199251", "module": "A1"}, {"value": "0.000322251461915386", "module": "A2"}, {"value": "0.0268180651283716", "module": "A3"}, {"value": "5.24596695848876E-05", "module": "A4"}, {"value": "0", "module": "A5"}, {"value": "0", "module": "C1"}, {"value": "1.02823398446905E-08", "module": "C2"}, {"value": "2.9988122202773E-06", "module": "C3"}, {"value": "0", "module": "C4"}, {"value": "-0.000138514637189766", "module": "D"}]}}, {"referenceToLCIAMethodDataSet": {"shortDescription": [{"value": "Toxizitätsvergleichseinheit für Ökosysteme (ETP-fw)", "lang": "de"}, {"value": "Comparative toxic unit for ecosystems (ETP-fw)", "lang": "en"}], "type": "LCIA method data set", "refObjectId": "ee1082d1-b0f7-43ca-a1f0-21e2a4a74511", "uri": "../lciamethods/ee1082d1-b0f7-43ca-a1f0-21e2a4a74511.xml"}, "other": {"anies": [{"name": "referenceToUnitGroupDataSet", "value": {"shortDescription": [{"value": "CTUe", "lang": "de"}], "type": "unit group data set", "refObjectId": "aa959ded-f1eb-4efb-9c5c-2d60be36b3e6", "uri": "../unitgroups/aa959ded-f1eb-4efb-9c5c-2d60be36b3e6.xml"}}, {"value": "6.40888049138785", "module": "A1"}, {"value": "1.21311512079813", "module": "A2"}, {"value": "0.386852274767684", "module": "A3"}, {"value": "0.365667766711459", "module": "A4"}, {"value": "0", "module": "A5"}, {"value": "0", "module": "C1"}, {"value": "3.87078521494944E-05", "module": "C2"}, {"value": "0.000110540050592439", "module": "C3"}, {"value": "0", "module": "C4"}, {"value": "-0.00471518225430689", "module": "D"}]}}, {"referenceToLCIAMethodDataSet": {"shortDescription": [{"value": "Toxizitätsvergleichseinheit für Menschen (krebserregend) (HTP-c)", "lang": "de"}, {"value": "Comparative toxic unit for humans (carcinogenic) (HTP-c)", "lang": "en"}], "type": "LCIA method data set", "refObjectId": "2299222a-bbd8-474f-9d4f-4dd1f18aea7c", "uri": "../lciamethods/2299222a-bbd8-474f-9d4f-4dd1f18aea7c.xml"}, "other": {"anies": [{"name": "referenceToUnitGroupDataSet", "value": {"shortDescription": [{"value": "CTUh", "lang": "de"}], "type": "unit group data set", "refObjectId": "d4c9523e-2d7e-49fd-8469-998f547d3a70", "uri": "../unitgroups/d4c9523e-2d7e-49fd-8469-998f547d3a70.xml"}}, {"value": "7.72947782633424E-09", "module": "A1"}, {"value": "2.45176649114131E-11", "module": "A2"}, {"value": "1.85990941503169E-11", "module": "A3"}, {"value": "7.22277102888615E-12", "module": "A4"}, {"value": "0", "module": "A5"}, {"value": "0", "module": "C1"}, {"value": "7.82305102105596E-16", "module": "C2"}, {"value": "5.66442062914322E-15", "module": "C3"}, {"value": "0", "module": "C4"}, {"value": "-3.47408050450445E-13", "module": "D"}]}}, {"referenceToLCIAMethodDataSet": {"shortDescription": [{"value": "Toxizitätsvergleichseinheit für Menschen (nicht krebserregend) (HTP-nc)", "lang": "de"}, {"value": "Comparative toxic unit for humans (noncarcinogenic) (HTP-nc)", "lang": "en"}], "type": "LCIA method data set", "refObjectId": "3af763a5-b7a1-48c9-9cee-1f223481fcef", "uri": "../lciamethods/3af763a5-b7a1-48c9-9cee-1f223481fcef.xml"}, "other": {"anies": [{"name": "referenceToUnitGroupDataSet", "value": {"shortDescription": [{"value": "CTUh", "lang": "de"}], "type": "unit group data set", "refObjectId": "d4c9523e-2d7e-49fd-8469-998f547d3a70", "uri": "../unitgroups/d4c9523e-2d7e-49fd-8469-998f547d3a70.xml"}}, {"value": "7.89508877527809E-09", "module": "A1"}, {"value": "1.0808569774921E-09", "module": "A2"}, {"value": "9.66267013935148E-10", "module": "A3"}, {"value": "2.98087849135221E-10", "module": "A4"}, {"value": "0", "module": "A5"}, {"value": "0", "module": "C1"}, {"value": "3.44877838568099E-14", "module": "C2"}, {"value": "7.92781420373562E-14", "module": "C3"}, {"value": "0", "module": "C4"}, {"value": "-7.55063967515881E-12", "module": "D"}]}}, {"referenceToLCIAMethodDataSet": {"shortDescription": [{"value": "Bodenqualitätsindex (SQP)", "lang": "de"}, {"value": "Soil quality index (SQP)", "lang": "en"}], "type": "LCIA method data set", "refObjectId": "b2ad6890-c78d-11e6-9d9d-cec0c932ce01", "uri": "../lciamethods/b2ad6890-c78d-11e6-9d9d-cec0c932ce01.xml"}, "other": {"anies": [{"name": "referenceToUnitGroupDataSet", "value": {"shortDescription": [{"value": "SQP", "lang": "de"}], "type": "unit group data set", "refObjectId": "f130951c-e67f-4f7f-8dd4-665de3974e18", "uri": "../unitgroups/f130951c-e67f-4f7f-8dd4-665de3974e18.xml"}}, {"value": "2.92995304144804", "module": "A1"}, {"value": "0.718682980629868", "module": "A2"}, {"value": "1.96504820252891", "module": "A3"}, {"value": "0.17282578410837", "module": "A4"}, {"value": "0", "module": "A5"}, {"value": "0", "module": "C1"}, {"value": "2.29316031756956E-05", "module": "C2"}, {"value": "0.000190188189630576", "module": "C3"}, {"value": "0", "module": "C4"}, {"value": "-0.00861566545301804", "module": "D"}]}}]}, "otherAttributes": {"{http://www.indata.network/EPD/2019}epd-version": "1.2"}, "version": "1.1", "locations": "../ILCDLocations.xml"}