{"processInformation": {"dataSetInformation": {"UUID": "006c17a5-bfbd-4786-8c96-7546e5317f9c", "name": {"baseName": [{"value": "SAGLAN Glaswolle, mit bio-basiertem Bindemittel +A2", "lang": "de"}, {"value": "SAGLAN glass wool, bonded with bio-based adhesive +A2", "lang": "en"}], "functionalUnitFlowProperties": [{"lang": "de"}]}, "classificationInformation": {"classification": [{"class": [{"value": "Dämmstoffe", "level": 0, "classId": "2"}, {"value": "Mineralwolle", "level": 1, "classId": "2.1"}, {"value": "Glaswolle", "level": 2, "classId": "2.1.02"}], "name": "OEKOBAU.DAT"}, {"class": [{"value": "02 Bauprodukte", "level": 0}, {"value": "Wärmedämmungsprodukte", "level": 1}, {"value": "Mineralische Dämmstoffe", "level": 2}], "name": "IBUCategories"}]}, "generalComment": [{"value": "Die Produktedeklaration bezieht sich auf Produkte aus Glaswolle. Glaswolle besteht aus künstlich hergestellten monofilen Mineralfasern nicht kristalliner Struktur. Der mittlere Faserdurchmesser beträgt zwischen 3 und 6 μm. Die Herstellung ist durch RAL und EUCEB überwacht und zertifiziert. Die Glaswolle entspricht der Definition der Glaswolle nach deutschem Gefahrstoffrecht. Die Rohdichte der SAGLAN-Produkte variiert von 12 bis 100 kg/m3. Die durchschnittliche Dichte der Produkte liegt bei rund 30 kg/m3. Die Produkte werden unter der Bezeichnung SAGLAN vertrieben. Sie sind in Rollenform oder als Platten im Handel erhältlich.", "lang": "de"}, {"value": "The product declaration refers to products made of glass wool. Glass wool consists of man-made monofilament mineral fibres of non-crystalline structure. The average fibre diameter is between 3 and 6 μm. The production is monitored and certified by RAL and EUCEB. The glass wool complies with the definition of glass wool according to German legislation on hazardous substances. The raw density of SAGLAN products varies from 12 to 100 kg/m3. The average density of the products is around 30 kg/m3.\n\nThe products are marketed under the name SAGLAN. They are commercially available in roll form or as slabs.", "lang": "en"}]}, "quantitativeReference": {"referenceToReferenceFlow": [0]}, "time": {"referenceYear": 2021, "dataSetValidUntil": 2026, "other": {"anies": [{"name": "publicationDateOfEPD", "value": 1612483200000}]}}, "geography": {"locationOfOperationSupplyOrProduction": {"location": "CH"}}, "technology": {"technologyDescriptionAndIncludedProcesses": [{"value": "unbeschichtete Glaswolle SAGLAN mit biobasiertem Bindemitte bei einer durchschnittlichen/typischen Dichte von 30 kg/m3. Glaswolle ist ein Dämmstoff aus Mineralwolle, dessen wesentlicher Bestandteil monofile künstliche Mineralfasern nichtkristalliner Struktur sind, die aus einer silikatischen Schmelze gewonnen werden. \nDeklarierte Einheit: \nDie deklarierten Werte beziehen sich auf 1 kg unbeschichtete SAGLAN Glaswolle mit bio-basiertem Bindemittel", "lang": "de"}, {"value": " \nDeclared unit: \nThe declared values refer to 1 kg of uncoated SAGLAN glass wool bonded with a bio-based adhesive.", "lang": "en"}], "technologicalApplicability": [{"value": "Die Anwendungsgebiete sind im Hochbau als thermische Dämmung von haustechnischen Installationen. Die Standardprodukte werden unter dem Namen SAGLAN gehandelt, jene für die Technik unter der Bezeichnung SAGLAN T.\n\nAls Wärmedämmung in Gebäuden werden die Platten oder Rollen zwischen der Tragkonstruktion im Dach-/Wand-/Zwischendecken- und Bodenbereich sowie innerhalb oder außerhalb der Tragkonstruktion eingebaut.\n\nAnwendungsbereich im Hochbau:\n\n\ndie Wärme- und Schalldämmung im Steildach und Flachdach.\n\nAufdachdämmung\n\nWärmedämmung von zweischaligen Mauerwerken\n\nWärmedämmung von hinterlüfteten Fassaden\n\nWärmedämmverbundsysteme\n\nHaustrennwände\n\nTrittschalldämmung in schwimmenden Estrichböden\n\nHolzrahmenbau\n\nHolzdecken\n\nKassettenwände\n\nInnendämmungen in Dach und Wand\n\nTrennlagen\n\nOberste Geschossdecke\n\nTiefgaragen und Kellerdecken\nAkustikdecken\n\nIm Bereich der Haustechnik:\n\nDämmung von Heizungen\n\nDämmung von Lüftungskanälen\n\nDämmung von Klimakanälen\n\nDämmung von Apparaturen\n\nDämmung von Rohrleitungen\n\nDämmung von Warmwasserspeichern\n\nDämmung von Tanks\n\nVerwendung bei industrieller Verarbeitung\n\nVerwendung in der Automotive\n\nVerwendung im Schiffbau\n\nVerwendung bei Brandschutzelementen\n\nVerarbeitung", "lang": "de"}, {"value": "The areas of application are in building construction as thermal insulation of building services installations. The standard products are marketed under the name SAGLAN, those for technical applications under the name SAGLAN T.\n\nAs thermal insulation in buildings, the slabs or rolls are installed between the supporting structure in the roof/wall/ceiling and floor area as well as inside or outside the supporting structure.\n\nField of application in building construction:\n\nThermal and sound insulation in pitched and flat roofs\nRooftop insulation\nThermal insulation of double-skin masonry walls\nThermal insulation of ventilated facades\nExternal thermal insulation composite systems\nInternal partition walls\nImpact sound insulation in floating screed floors\nTimber frame construction\nWooden ceilings\nCassette walls\nInterior insulation in roof and wall\nSeparating layers\nUpper storey ceiling\nUnderground garages and basement ceilings\nAcoustic ceilings\n\n\n\nIn the area of building services:\n\nInsulation of heating systems\nInsulation of ventilation ducts\nInsulation of air conditioning ducts\nInsulation of apparatus\nInsulation of pipelines\nInsulation of hot water tanks\nInsulation of tanks\nUse in industrial processing\nUse in the automotive industry\nUse in shipbuilding\nUse with fire protection elements\nProcessing", "lang": "en"}]}}, "modellingAndValidation": {"LCIMethodAndAllocation": {"typeOfDataSet": "EPD", "referenceToLCAMethodDetails": [{"shortDescription": [{"value": "Mineralische Dämmstoffe.pdf", "lang": "de"}], "type": "source data set", "refObjectId": "64094d77-fcbe-48fd-b2cc-e201c9df29ac"}], "other": {"anies": [{"name": "subType", "value": "specific dataset"}]}}, "dataSourcesTreatmentAndRepresentativeness": {"referenceToDataSource": [{"shortDescription": [{"value": "ecoinvent database (all versions)", "lang": "de"}], "type": "source data set", "refObjectId": "b497a91f-e14b-4b69-8f28-f50eb1576766"}, {"shortDescription": [{"value": "ecoinvent 2.2 database", "lang": "de"}], "type": "source data set", "refObjectId": "9ffadc15-4649-4871-b565-cee8197b17e9"}], "useAdviceForDataSet": [{"value": "Gültigkeitsbereich: \nDie Deklaration bezieht sich auf SAGLAN Glaswolle, die am Standort der Sager AG in Dürrenäsch/CH hergestellt wird. \nSystemgrenze: \nTyp der EPD: Wiege bis Werkstor – mit Optionen\n\nDie Module A1–A3 umfassen sämtliche Stoff- und Energieflüsse, die für die Herstellung von SAGLAN Glaswolle benötigt werden; die Systemgrenze für Altglas wird an dem Punkt angenommen, an dem es sortenrein vorliegt.\n\nModul A4 umfasst den Transport auf die Baustelle.\n\nModul A5 umfasst die Verbrennung der Transportverpackungen in einer Kehrichtverbrennungsanlage (KVA), wobei die rückgewonnene Energie in Modul D exportiert wird.\n\nZusätzlich werden in Anlehnung an EN 16783 2% Verschnitt angenommen, womit eine entsprechende Produktionsmenge inkl. Verpackung und Transport auf die Baustelle und deren Entsorgung (Verschnitt und dessen Verpackung) in Modul A5 mitbilanziert werden.\n\nModul C1: während des Rückbaus werden Staubemissionen bilanziert.\n\nModul C2 umfasst den Transport der rückgebauten Glaswolle auf eine Inertstoffdeponie.\n\nModul C3: aufgrund des angenommenen Entsorgungsszenarios in einer Inertstoffdeponie fallen in diesem Modul keine Umweltwirkungen an.\n\nModul C4 umfasst den Deponierungsprozess von Glaswolle ohne die Berücksichtigung der energetischen Nutzung des Deponiegases aus den (geringen) organischen Bestandteilen.\n\nModul D umfasst die Gutschriften aus der Produktion von Strom und Wärme, die bei der thermischen Behandlung der Verpackungsabfälle aus dem Einbau der Glaswolle auf der Baustelle (inkl. 2 % der Verpackung des Verschnitts) aus Modul A5 in einer KVA erzeugt werden.", "lang": "de"}, {"value": "Scope: \nThe declaration refers to SAGLAN glass wool, which is manufactured at the Sager AG site in Dürrenäsch/CH. \nSystem boundary: \nType of EPD: Cradle to factory gate - with options\n\nModules A1-A3 cover all material and energy flows required for the production of SAGLAN glass wool; the system boundary for waste glass is assumed to be at the point where it is sorted by type.\n\nModule A4 includes transport to the construction site. \n\nModule A5 involves the incineration of the transport packaging in a waste incineration plant (MWIP), with the recovered energy being exported to Module D.\n\nIn addition, 2% waste is assumed in accordance with EN 16783, which means that a corresponding production quantity including packaging and transport to the construction site and its disposal (waste and its packaging) are also inventoried in module A5.\n\nModule C1: dust emissions are inventoried during deconstruction.\n\nModule C2 comprises the transport of the deconstructed glass wool to a landfill for inert materials.\n\nIn Module C3, due to the assumed disposal scenario in an inert landfill, no environmental impacts occur in this module.\n\nModule C4 covers the landfilling process of glass wool without taking into account the energetic utilisation of the landfill gas from the (small) organic components.\n\nModule D includes the benefits from the production of electricity and heat generated from the thermal treatment of the packaging waste from the installation of the glass wool on the construction site (incl. 2 % of the packaging offcuts) from Module A5 in a MWIP.", "lang": "en"}], "other": {"anies": [{"name": "referenceToOriginalEPD", "value": {"shortDescription": {"value": "SAGLAN Glaswolle, mit bio-basiertem Bindemittel +A2.pdf", "defaultValue": "SAGLAN Glaswolle, mit bio-basiertem Bindemittel +A2.pdf", "lstrings": [{"lang": "de", "value": "SAGLAN Glaswolle, mit bio-basiertem Bindemittel +A2.pdf"}]}, "type": "source data set", "uuid": {"uuid": "dfa112b4-cbb4-4710-a4e6-6fcd2b921f9b"}, "refObjectId": "dfa112b4-cbb4-4710-a4e6-6fcd2b921f9b", "resourceURLs": ["https://oekobaudat.de/OEKOBAU.DAT/resource/sources/dfa112b4-cbb4-4710-a4e6-6fcd2b921f9b/SAGLAN_Glaswolle_mit_bio-basiertem_Bindemittel_A2_13201.pdf?version=00.01.000"]}}]}}, "validation": {"review": [{"referenceToNameOfReviewerAndInstitution": [{"shortDescription": [{"value": "Institut Bauen und Umwelt e. V.", "lang": "de"}], "type": "contact data set", "refObjectId": "d111dbec-b024-4be5-86c5-752d6eb2cf95", "uri": "../contacts/d111dbec-b024-4be5-86c5-752d6eb2cf95.xml"}], "type": "Accredited third party review"}]}, "complianceDeclarations": {"compliance": [{"referenceToComplianceSystem": {"shortDescription": [{"value": "DIN EN 15804+A2", "lang": "de"}], "type": "source data set", "refObjectId": "c0016b33-8cf7-415c-ac6e-deba0d21440d", "uri": "../sources/c0016b33-8cf7-415c-ac6e-deba0d21440d.xml"}}, {"referenceToComplianceSystem": {"shortDescription": [{"value": "ISO 14025", "lang": "de"}], "type": "source data set", "refObjectId": "4f2eb655-6e44-4874-a95a-e28f5442cd4d", "uri": "../sources/4f2eb655-6e44-4874-a95a-e28f5442cd4d.xml"}}]}}, "administrativeInformation": {"commissionerAndGoal": {"referenceToCommissioner": [{"shortDescription": [{"value": "Sager AG", "lang": "de"}], "type": "contact data set", "refObjectId": "cb72c4c2-4155-4e7d-b45c-dc20c56c552a", "uri": "../contacts/cb72c4c2-4155-4e7d-b45c-dc20c56c552a.xml"}]}, "dataGenerator": {"referenceToPersonOrEntityGeneratingTheDataSet": [{"shortDescription": [{"value": "Dr. Frank Werner - Umwelt & Entwicklung", "lang": "de"}], "type": "contact data set", "refObjectId": "62792478-795c-4ae2-ac9a-1012d9515424", "uri": "../contacts/62792478-795c-4ae2-ac9a-1012d9515424.xml"}]}, "dataEntryBy": {"timeStamp": 1612519843262, "referenceToDataSetFormat": [{"shortDescription": [{"value": "ILCD Format", "lang": "de"}], "type": "source data set", "refObjectId": "a97a0155-0234-4b87-b4ce-a45da52f2a40", "uri": "../sources/a97a0155-0234-4b87-b4ce-a45da52f2a40.xml"}, {"shortDescription": [{"value": "EPD-Datenformaterweiterungen v1.2", "lang": "de"}, {"value": "EPD Data Format Extensions v1.2", "lang": "en"}], "type": "source data set", "refObjectId": "a29449fd-aa2f-4de8-b5d7-4b06b43c6fde", "uri": "../sources/a29449fd-aa2f-4de8-b5d7-4b06b43c6fde.xml"}]}, "publicationAndOwnership": {"dataSetVersion": "00.01.000", "referenceToRegistrationAuthority": {"shortDescription": [{"value": "Institut Bauen und Umwelt e. V.", "lang": "de"}], "type": "contact data set", "refObjectId": "d111dbec-b024-4be5-86c5-752d6eb2cf95", "uri": "../contacts/d111dbec-b024-4be5-86c5-752d6eb2cf95.xml"}, "registrationNumber": "EPD-SAR-20200274-CBA1-DE", "referenceToOwnershipOfDataSet": {"shortDescription": [{"value": "Sager AG", "lang": "de"}], "type": "contact data set", "refObjectId": "cb72c4c2-4155-4e7d-b45c-dc20c56c552a", "uri": "../contacts/cb72c4c2-4155-4e7d-b45c-dc20c56c552a.xml"}, "copyright": true, "licenseType": "Free of charge for all users and uses", "accessRestrictions": [{"value": "None", "lang": "en"}], "other": {"anies": [{"name": "referenceToPublisher", "value": {"shortDescription": [{"value": "Institut Bauen und Umwelt e. V.", "lang": "de"}], "type": "contact data set", "refObjectId": "d111dbec-b024-4be5-86c5-752d6eb2cf95", "uri": "../contacts/d111dbec-b024-4be5-86c5-752d6eb2cf95.xml"}}]}}}, "exchanges": {"exchange": [{"dataSetInternalID": 0, "referenceToFlowDataSet": {"shortDescription": [{"value": "SAGLAN Glaswolle, mit bio-basiertem Bindemittel ()", "lang": "de"}], "type": "flow data set", "refObjectId": "8f6f877c-b7bd-beb7-90ea-92a937d55638", "uri": "../flows/8f6f877c-b7bd-beb7-90ea-92a937d55638.xml"}, "meanAmount": 1.0, "referencesToDataSource": {}, "referenceFlow": true, "resolvedFlowVersion": "00.01.000", "resultingflowAmount": 1.0, "flowProperties": [{"name": [{"lang": "en", "value": "Mass"}, {"lang": "de", "value": "Masse"}], "uuid": "93a60a56-a3c8-11da-a746-0800200b9a66", "referenceFlowProperty": true, "meanValue": 1.0, "referenceUnit": "kg", "unitGroupUUID": "ad38d542-3fe9-439d-9b95-2f5f7752acaf"}], "materialProperties": [{"name": "conversion factor [mass/declared unit]", "value": "1.0", "unit": "-", "unitDescription": "Without unit"}, {"name": "gross density", "value": "30.0", "unit": "kg/m^3", "unitDescription": "kilograms per cubic metre"}], "typeOfFlow": "Product flow", "classification": {"classHierarchy": "Dämmstoffe / Mineralwolle / Glaswolle", "name": "OEKOBAU.DAT"}}, {"dataSetInternalID": 1, "referenceToFlowDataSet": {"shortDescription": [{"value": "Erneuerbare Primärenergie als Energieträger (PERE)", "lang": "de"}, {"value": "Renewable primary energy as energy carrier (PERE)", "lang": "en"}], "type": "flow data set", "refObjectId": "20f32be5-0398-4288-9b6d-accddd195317", "uri": "../flows/20f32be5-0398-4288-9b6d-accddd195317.xml"}, "exchange direction": "INPUT", "other": {"anies": [{"name": "referenceToUnitGroupDataSet", "value": {"shortDescription": [{"value": "MJ", "lang": "de"}], "type": "unit group data set", "refObjectId": "93a60a57-a3c8-11da-a746-0800200c9a66", "uri": "../unitgroups/93a60a57-a3c8-11da-a746-0800200c9a66.xml"}}, {"value": "4.71747912728004", "module": "A1-A3"}, {"value": "0.00558014898714353", "module": "A4"}, {"value": "0.0899273800337747", "module": "A5"}, {"value": "0", "module": "C1"}, {"value": "0.000479580718775214", "module": "C2"}, {"value": "0", "module": "C3"}, {"value": "0.0017206630714221", "module": "C4"}, {"value": "-0.157734061730717", "module": "D"}]}, "resolvedFlowVersion": "38.00.000", "flowProperties": [], "typeOfFlow": "Other flow", "classification": {"classHierarchy": "Quantities", "name": "GaBiCategories"}}, {"dataSetInternalID": 2, "referenceToFlowDataSet": {"shortDescription": [{"value": "Erneuerbare Primärenergie zur stofflichen Nutzung (PERM)", "lang": "de"}, {"value": "Renewable primary energy resources as material utilization (PERM)", "lang": "en"}], "type": "flow data set", "refObjectId": "fb3ec0de-548d-4508-aea5-00b73bf6f702", "uri": "../flows/fb3ec0de-548d-4508-aea5-00b73bf6f702.xml"}, "exchange direction": "INPUT", "other": {"anies": [{"name": "referenceToUnitGroupDataSet", "value": {"shortDescription": [{"value": "MJ", "lang": "de"}], "type": "unit group data set", "refObjectId": "93a60a57-a3c8-11da-a746-0800200c9a66", "uri": "../unitgroups/93a60a57-a3c8-11da-a746-0800200c9a66.xml"}}, {"value": "0", "module": "A1-A3"}, {"value": "0", "module": "A4"}, {"value": "0", "module": "A5"}, {"value": "0", "module": "C1"}, {"value": "0", "module": "C2"}, {"value": "0", "module": "C3"}, {"value": "0", "module": "C4"}, {"value": "0", "module": "D"}]}, "resolvedFlowVersion": "38.00.000", "flowProperties": [], "typeOfFlow": "Other flow", "classification": {"classHierarchy": "Quantities", "name": "GaBiCategories"}}, {"dataSetInternalID": 3, "referenceToFlowDataSet": {"shortDescription": [{"value": "Total erneuerbare Primärenergie (PERT)", "lang": "de"}, {"value": "Total use of renewable primary energy resources (PERT)", "lang": "en"}], "type": "flow data set", "refObjectId": "53f97275-fa8a-4cdd-9024-65936002acd0", "uri": "../flows/53f97275-fa8a-4cdd-9024-65936002acd0.xml"}, "exchange direction": "INPUT", "other": {"anies": [{"name": "referenceToUnitGroupDataSet", "value": {"shortDescription": [{"value": "MJ", "lang": "de"}], "type": "unit group data set", "refObjectId": "93a60a57-a3c8-11da-a746-0800200c9a66", "uri": "../unitgroups/93a60a57-a3c8-11da-a746-0800200c9a66.xml"}}, {"value": "4.71747912728004", "module": "A1-A3"}, {"value": "0.00558014898714353", "module": "A4"}, {"value": "0.0899273800337747", "module": "A5"}, {"value": "0", "module": "C1"}, {"value": "0.000479580718775214", "module": "C2"}, {"value": "0", "module": "C3"}, {"value": "0.0017206630714221", "module": "C4"}, {"value": "-0.157734061730717", "module": "D"}]}, "resolvedFlowVersion": "38.00.000", "flowProperties": [], "typeOfFlow": "Other flow", "classification": {"classHierarchy": "Quantities / Environmental quantities / EPD EN 15804 / LCI indicators", "name": "GaBiCategories"}}, {"dataSetInternalID": 4, "referenceToFlowDataSet": {"shortDescription": [{"value": "Nicht-erneuerbare Primärenergie als Energieträger (PENRE)", "lang": "de"}, {"value": "Non renewable primary energy as energy carrier (PENRE)", "lang": "en"}], "type": "flow data set", "refObjectId": "ac857178-2b45-46ec-892a-a9a4332f0372", "uri": "../flows/ac857178-2b45-46ec-892a-a9a4332f0372.xml"}, "exchange direction": "INPUT", "other": {"anies": [{"name": "referenceToUnitGroupDataSet", "value": {"shortDescription": [{"value": "MJ", "lang": "de"}], "type": "unit group data set", "refObjectId": "93a60a57-a3c8-11da-a746-0800200c9a66", "uri": "../unitgroups/93a60a57-a3c8-11da-a746-0800200c9a66.xml"}}, {"value": "27.1182696685828", "module": "A1-A3"}, {"value": "0.379720008945126", "module": "A4"}, {"value": "0.744999673446038", "module": "A5"}, {"value": "0", "module": "C1"}, {"value": "0.0326346832750883", "module": "C2"}, {"value": "0", "module": "C3"}, {"value": "0.183966550493215", "module": "C4"}, {"value": "-1.45897544812302", "module": "D"}]}, "resolvedFlowVersion": "38.00.000", "flowProperties": [], "typeOfFlow": "Other flow", "classification": {"classHierarchy": "Quantities", "name": "GaBiCategories"}}, {"dataSetInternalID": 5, "referenceToFlowDataSet": {"shortDescription": [{"value": "Nicht-erneuerbare Primärenergie zur stofflichen Nutzung (PENRM)", "lang": "de"}, {"value": "Non renewable primary energy as material utilization (PENRM)", "lang": "en"}], "type": "flow data set", "refObjectId": "1421caa0-679d-4bf4-b282-0eb850ccae27", "uri": "../flows/1421caa0-679d-4bf4-b282-0eb850ccae27.xml"}, "exchange direction": "INPUT", "other": {"anies": [{"name": "referenceToUnitGroupDataSet", "value": {"shortDescription": [{"value": "MJ", "lang": "de"}], "type": "unit group data set", "refObjectId": "93a60a57-a3c8-11da-a746-0800200c9a66", "uri": "../unitgroups/93a60a57-a3c8-11da-a746-0800200c9a66.xml"}}, {"value": "0", "module": "A1-A3"}, {"value": "0", "module": "A4"}, {"value": "0", "module": "A5"}, {"value": "0", "module": "C1"}, {"value": "0", "module": "C2"}, {"value": "0", "module": "C3"}, {"value": "0", "module": "C4"}, {"value": "0", "module": "D"}]}, "resolvedFlowVersion": "38.00.000", "flowProperties": [], "typeOfFlow": "Other flow", "classification": {"classHierarchy": "Quantities", "name": "GaBiCategories"}}, {"dataSetInternalID": 6, "referenceToFlowDataSet": {"shortDescription": [{"value": "Total nicht erneuerbare Primärenergie (PENRT)", "lang": "de"}, {"value": "Total use of non renewable primary energy resources (PENRT)", "lang": "en"}], "type": "flow data set", "refObjectId": "06159210-646b-4c8d-8583-da9b3b95a6c1", "uri": "../flows/06159210-646b-4c8d-8583-da9b3b95a6c1.xml"}, "exchange direction": "INPUT", "other": {"anies": [{"name": "referenceToUnitGroupDataSet", "value": {"shortDescription": [{"value": "MJ", "lang": "de"}], "type": "unit group data set", "refObjectId": "93a60a57-a3c8-11da-a746-0800200c9a66", "uri": "../unitgroups/93a60a57-a3c8-11da-a746-0800200c9a66.xml"}}, {"value": "27.1182696685828", "module": "A1-A3"}, {"value": "0.379720008945126", "module": "A4"}, {"value": "0.744999673446038", "module": "A5"}, {"value": "0", "module": "C1"}, {"value": "0.0326346832750883", "module": "C2"}, {"value": "0", "module": "C3"}, {"value": "0.183966550493215", "module": "C4"}, {"value": "-1.45897544812302", "module": "D"}]}, "resolvedFlowVersion": "38.00.000", "flowProperties": [], "typeOfFlow": "Other flow", "classification": {"classHierarchy": "Quantities / Environmental quantities / EPD EN 15804 / LCI indicators", "name": "GaBiCategories"}}, {"dataSetInternalID": 7, "referenceToFlowDataSet": {"shortDescription": [{"value": "Einsatz von Sekundärstoffen (SM)", "lang": "de"}, {"value": "Use of secondary material (SM)", "lang": "en"}], "type": "flow data set", "refObjectId": "c6a1f35f-2d09-4f54-8dfb-97e502e1ce92", "uri": "../flows/c6a1f35f-2d09-4f54-8dfb-97e502e1ce92.xml"}, "exchange direction": "INPUT", "other": {"anies": [{"name": "referenceToUnitGroupDataSet", "value": {"shortDescription": [{"value": "kg", "lang": "de"}], "type": "unit group data set", "refObjectId": "ad38d542-3fe9-439d-9b95-2f5f7752acaf", "uri": "../unitgroups/ad38d542-3fe9-439d-9b95-2f5f7752acaf.xml"}}, {"value": "0.75", "module": "A1-A3"}, {"value": "0", "module": "A4"}, {"value": "0.015", "module": "A5"}, {"value": "0", "module": "C1"}, {"value": "0", "module": "C2"}, {"value": "0", "module": "C3"}, {"value": "0", "module": "C4"}, {"value": "0", "module": "D"}]}, "resolvedFlowVersion": "38.00.000", "flowProperties": [], "typeOfFlow": "Other flow", "classification": {"classHierarchy": "Quantities / Environmental quantities / EPD EN 15804 / LCI indicators", "name": "GaBiCategories"}}, {"dataSetInternalID": 8, "referenceToFlowDataSet": {"shortDescription": [{"value": "Erneuerbare Sekundärbrennstoffe (RSF)", "lang": "de"}, {"value": "Use of renewable secondary fuels (RSF)", "lang": "en"}], "type": "flow data set", "refObjectId": "64333088-a55f-4aa2-9a31-c10b07816787", "uri": "../flows/64333088-a55f-4aa2-9a31-c10b07816787.xml"}, "exchange direction": "INPUT", "other": {"anies": [{"name": "referenceToUnitGroupDataSet", "value": {"shortDescription": [{"value": "MJ", "lang": "de"}], "type": "unit group data set", "refObjectId": "93a60a57-a3c8-11da-a746-0800200c9a66", "uri": "../unitgroups/93a60a57-a3c8-11da-a746-0800200c9a66.xml"}}, {"value": "0", "module": "A1-A3"}, {"value": "0", "module": "A4"}, {"value": "0", "module": "A5"}, {"value": "0", "module": "C1"}, {"value": "0", "module": "C2"}, {"value": "0", "module": "C3"}, {"value": "0", "module": "C4"}, {"value": "0", "module": "D"}]}, "resolvedFlowVersion": "38.00.000", "flowProperties": [], "typeOfFlow": "Other flow", "classification": {"classHierarchy": "Quantities / Environmental quantities / EPD EN 15804 / LCI indicators", "name": "GaBiCategories"}}, {"dataSetInternalID": 9, "referenceToFlowDataSet": {"shortDescription": [{"value": "Nicht erneuerbare Sekundärbrennstoffe (NRSF)", "lang": "de"}, {"value": "Use of non renewable secondary fuels (NRSF)", "lang": "en"}], "type": "flow data set", "refObjectId": "89def144-d39a-4287-b86f-efde453ddcb2", "uri": "../flows/89def144-d39a-4287-b86f-efde453ddcb2.xml"}, "exchange direction": "INPUT", "other": {"anies": [{"name": "referenceToUnitGroupDataSet", "value": {"shortDescription": [{"value": "MJ", "lang": "de"}], "type": "unit group data set", "refObjectId": "93a60a57-a3c8-11da-a746-0800200c9a66", "uri": "../unitgroups/93a60a57-a3c8-11da-a746-0800200c9a66.xml"}}, {"value": "0", "module": "A1-A3"}, {"value": "0", "module": "A4"}, {"value": "0", "module": "A5"}, {"value": "0", "module": "C1"}, {"value": "0", "module": "C2"}, {"value": "0", "module": "C3"}, {"value": "0", "module": "C4"}, {"value": "0", "module": "D"}]}, "resolvedFlowVersion": "38.00.000", "flowProperties": [], "typeOfFlow": "Other flow", "classification": {"classHierarchy": "Quantities / Environmental quantities / EPD EN 15804 / LCI indicators", "name": "GaBiCategories"}}, {"dataSetInternalID": 10, "referenceToFlowDataSet": {"shortDescription": [{"value": "Einsatz von Süßwasserressourcen (FW)", "lang": "de"}, {"value": "Use of net fresh water (FW)", "lang": "en"}], "type": "flow data set", "refObjectId": "3cf952c8-f3a4-461d-8c96-96456ca62246", "uri": "../flows/3cf952c8-f3a4-461d-8c96-96456ca62246.xml"}, "exchange direction": "INPUT", "other": {"anies": [{"name": "referenceToUnitGroupDataSet", "value": {"shortDescription": [{"value": "m^3", "lang": "de"}], "type": "unit group data set", "refObjectId": "cd950537-0a98-4044-9ba7-9f9a68d0a504", "uri": "../unitgroups/cd950537-0a98-4044-9ba7-9f9a68d0a504.xml"}}, {"value": "0.0227095570749073", "module": "A1-A3"}, {"value": "0.00017717970455767", "module": "A4"}, {"value": "0.000813863721849241", "module": "A5"}, {"value": "0", "module": "C1"}, {"value": "1.52275450458258E-05", "module": "C2"}, {"value": "0", "module": "C3"}, {"value": "0.000198592057832039", "module": "C4"}, {"value": "-0.000682451282256431", "module": "D"}]}, "resolvedFlowVersion": "38.00.000", "flowProperties": [], "typeOfFlow": "Other flow", "classification": {"classHierarchy": "Quantities / Environmental quantities / EPD EN 15804 / LCI indicators", "name": "GaBiCategories"}}, {"dataSetInternalID": 11, "referenceToFlowDataSet": {"shortDescription": [{"value": "Gefährlicher Abfall zur Deponie (HWD)", "lang": "de"}, {"value": "Hazardous waste disposed (HWD)", "lang": "en"}], "type": "flow data set", "refObjectId": "430f9e0f-59b2-46a0-8e0d-55e0e84948fc", "uri": "../flows/430f9e0f-59b2-46a0-8e0d-55e0e84948fc.xml"}, "exchange direction": "OUTPUT", "other": {"anies": [{"name": "referenceToUnitGroupDataSet", "value": {"shortDescription": [{"value": "kg", "lang": "de"}], "type": "unit group data set", "refObjectId": "ad38d542-3fe9-439d-9b95-2f5f7752acaf", "uri": "../unitgroups/ad38d542-3fe9-439d-9b95-2f5f7752acaf.xml"}}, {"value": "2.31818293639151E-05", "module": "A1-A3"}, {"value": "4.30181916274639E-07", "module": "A4"}, {"value": "7.09458035888105E-07", "module": "A5"}, {"value": "0", "module": "C1"}, {"value": "3.69715850036288E-08", "module": "C2"}, {"value": "0", "module": "C3"}, {"value": "6.25569617068109E-08", "module": "C4"}, {"value": "-5.04602495609112E-07", "module": "D"}]}, "resolvedFlowVersion": "38.00.000", "flowProperties": [], "typeOfFlow": "Other flow", "classification": {"classHierarchy": "Quantities / Environmental quantities / EPD EN 15804 / LCI indicators", "name": "GaBiCategories"}}, {"dataSetInternalID": 12, "referenceToFlowDataSet": {"shortDescription": [{"value": "Entsorgter nicht gefährlicher Abfall (NHWD)", "lang": "de"}, {"value": "Non hazardous waste disposed (NHWD)", "lang": "en"}], "type": "flow data set", "refObjectId": "b29ef66b-e286-4afa-949f-62f1a7b4d7fa", "uri": "../flows/b29ef66b-e286-4afa-949f-62f1a7b4d7fa.xml"}, "exchange direction": "OUTPUT", "other": {"anies": [{"name": "referenceToUnitGroupDataSet", "value": {"shortDescription": [{"value": "kg", "lang": "de"}], "type": "unit group data set", "refObjectId": "ad38d542-3fe9-439d-9b95-2f5f7752acaf", "uri": "../unitgroups/ad38d542-3fe9-439d-9b95-2f5f7752acaf.xml"}}, {"value": "0.186376443836701", "module": "A1-A3"}, {"value": "0.00335432632437745", "module": "A4"}, {"value": "0.0296665559417367", "module": "A5"}, {"value": "0", "module": "C1"}, {"value": "0.000288284458597411", "module": "C2"}, {"value": "0", "module": "C3"}, {"value": "0.999438279801346", "module": "C4"}, {"value": "-0.00156169202577969", "module": "D"}]}, "resolvedFlowVersion": "38.00.000", "flowProperties": [], "typeOfFlow": "Other flow", "classification": {"classHierarchy": "Quantities / Environmental quantities / EPD EN 15804 / LCI indicators", "name": "GaBiCategories"}}, {"dataSetInternalID": 13, "referenceToFlowDataSet": {"shortDescription": [{"value": "Entsorgter radioaktiver Abfall (RWD)", "lang": "de"}, {"value": "Radioactive waste disposed (RWD)", "lang": "en"}], "type": "flow data set", "refObjectId": "3449546e-52ad-4b39-b809-9fb77cea8ff6", "uri": "../flows/3449546e-52ad-4b39-b809-9fb77cea8ff6.xml"}, "exchange direction": "OUTPUT", "other": {"anies": [{"name": "referenceToUnitGroupDataSet", "value": {"shortDescription": [{"value": "kg", "lang": "de"}], "type": "unit group data set", "refObjectId": "ad38d542-3fe9-439d-9b95-2f5f7752acaf", "uri": "../unitgroups/ad38d542-3fe9-439d-9b95-2f5f7752acaf.xml"}}, {"value": "0.000244528392188667", "module": "A1-A3"}, {"value": "4.23744198499695E-07", "module": "A4"}, {"value": "5.11919033467685E-06", "module": "A5"}, {"value": "0", "module": "C1"}, {"value": "3.64183013323697E-08", "module": "C2"}, {"value": "0", "module": "C3"}, {"value": "1.31905135594573E-07", "module": "C4"}, {"value": "-1.47231530713134E-05", "module": "D"}]}, "resolvedFlowVersion": "38.00.000", "flowProperties": [], "typeOfFlow": "Other flow", "classification": {"classHierarchy": "Quantities / Environmental quantities / EPD EN 15804 / LCI indicators", "name": "GaBiCategories"}}, {"dataSetInternalID": 14, "referenceToFlowDataSet": {"shortDescription": [{"value": "Komponenten für die Wiederverwendung (CRU)", "lang": "de"}, {"value": "Components for re-use (CRU)", "lang": "en"}], "type": "flow data set", "refObjectId": "a2b32f97-3fc7-4af2-b209-525bc6426f33", "uri": "../flows/a2b32f97-3fc7-4af2-b209-525bc6426f33.xml"}, "exchange direction": "OUTPUT", "other": {"anies": [{"name": "referenceToUnitGroupDataSet", "value": {"shortDescription": [{"value": "kg", "lang": "de"}], "type": "unit group data set", "refObjectId": "ad38d542-3fe9-439d-9b95-2f5f7752acaf", "uri": "../unitgroups/ad38d542-3fe9-439d-9b95-2f5f7752acaf.xml"}}, {"value": "0", "module": "A1-A3"}, {"value": "0", "module": "A4"}, {"value": "0", "module": "A5"}, {"value": "0", "module": "C1"}, {"value": "0", "module": "C2"}, {"value": "0", "module": "C3"}, {"value": "0", "module": "C4"}, {"value": "0", "module": "D"}]}, "resolvedFlowVersion": "38.00.000", "flowProperties": [], "typeOfFlow": "Other flow", "classification": {"classHierarchy": "Quantities / Environmental quantities / EPD EN 15804 / LCI indicators", "name": "GaBiCategories"}}, {"dataSetInternalID": 15, "referenceToFlowDataSet": {"shortDescription": [{"value": "Stoffe zum Recycling (MFR)", "lang": "de"}, {"value": "Materials for recycling (MFR)", "lang": "en"}], "type": "flow data set", "refObjectId": "d7fe48a5-4103-49c8-9aae-b0b5dfdbd6ae", "uri": "../flows/d7fe48a5-4103-49c8-9aae-b0b5dfdbd6ae.xml"}, "exchange direction": "OUTPUT", "other": {"anies": [{"name": "referenceToUnitGroupDataSet", "value": {"shortDescription": [{"value": "kg", "lang": "de"}], "type": "unit group data set", "refObjectId": "ad38d542-3fe9-439d-9b95-2f5f7752acaf", "uri": "../unitgroups/ad38d542-3fe9-439d-9b95-2f5f7752acaf.xml"}}, {"value": "0", "module": "A1-A3"}, {"value": "0", "module": "A4"}, {"value": "0", "module": "A5"}, {"value": "0", "module": "C1"}, {"value": "0", "module": "C2"}, {"value": "0", "module": "C3"}, {"value": "0", "module": "C4"}, {"value": "0", "module": "D"}]}, "resolvedFlowVersion": "38.00.000", "flowProperties": [], "typeOfFlow": "Other flow", "classification": {"classHierarchy": "Quantities / Environmental quantities / EPD EN 15804 / LCI indicators", "name": "GaBiCategories"}}, {"dataSetInternalID": 16, "referenceToFlowDataSet": {"shortDescription": [{"value": "Stoffe für die Energierückgewinnung (MER)", "lang": "de"}, {"value": "Materials for energy recovery (MER)", "lang": "en"}], "type": "flow data set", "refObjectId": "59a9181c-3aaf-46ee-8b13-2b3723b6e447", "uri": "../flows/59a9181c-3aaf-46ee-8b13-2b3723b6e447.xml"}, "exchange direction": "OUTPUT", "other": {"anies": [{"name": "referenceToUnitGroupDataSet", "value": {"shortDescription": [{"value": "kg", "lang": "de"}], "type": "unit group data set", "refObjectId": "ad38d542-3fe9-439d-9b95-2f5f7752acaf", "uri": "../unitgroups/ad38d542-3fe9-439d-9b95-2f5f7752acaf.xml"}}, {"value": "0", "module": "A1-A3"}, {"value": "0", "module": "A4"}, {"value": "0", "module": "A5"}, {"value": "0", "module": "C1"}, {"value": "0", "module": "C2"}, {"value": "0", "module": "C3"}, {"value": "0", "module": "C4"}, {"value": "0", "module": "D"}]}, "resolvedFlowVersion": "38.00.000", "flowProperties": [], "typeOfFlow": "Other flow", "classification": {"classHierarchy": "Quantities / Environmental quantities / EPD EN 15804 / LCI indicators", "name": "GaBiCategories"}}, {"dataSetInternalID": 17, "referenceToFlowDataSet": {"shortDescription": [{"value": "Exportierte elektrische Energie (EEE)", "lang": "de"}, {"value": "Exported electrical energy (EEE)", "lang": "en"}], "type": "flow data set", "refObjectId": "4da0c987-2b76-40d6-9e9e-82a017aaaf29", "uri": "../flows/4da0c987-2b76-40d6-9e9e-82a017aaaf29.xml"}, "exchange direction": "OUTPUT", "other": {"anies": [{"name": "referenceToUnitGroupDataSet", "value": {"shortDescription": [{"value": "MJ", "lang": "de"}], "type": "unit group data set", "refObjectId": "93a60a57-a3c8-11da-a746-0800200c9a66", "uri": "../unitgroups/93a60a57-a3c8-11da-a746-0800200c9a66.xml"}}, {"value": "0", "module": "A1-A3"}, {"value": "0", "module": "A4"}, {"value": "0.3389256", "module": "A5"}, {"value": "0", "module": "C1"}, {"value": "0", "module": "C2"}, {"value": "0", "module": "C3"}, {"value": "0", "module": "C4"}, {"value": "0", "module": "D"}]}, "resolvedFlowVersion": "38.00.000", "flowProperties": [], "typeOfFlow": "Other flow", "classification": {"classHierarchy": "Quantities / Environmental quantities / EPD EN 15804 / LCI indicators", "name": "GaBiCategories"}}, {"dataSetInternalID": 18, "referenceToFlowDataSet": {"shortDescription": [{"value": "Exportierte thermische Energie (EET)", "lang": "de"}, {"value": "Exported thermal energy (EET)", "lang": "en"}], "type": "flow data set", "refObjectId": "98daf38a-7a79-46d3-9a37-2b7bd0955810", "uri": "../flows/98daf38a-7a79-46d3-9a37-2b7bd0955810.xml"}, "exchange direction": "OUTPUT", "other": {"anies": [{"name": "referenceToUnitGroupDataSet", "value": {"shortDescription": [{"value": "MJ", "lang": "de"}], "type": "unit group data set", "refObjectId": "93a60a57-a3c8-11da-a746-0800200c9a66", "uri": "../unitgroups/93a60a57-a3c8-11da-a746-0800200c9a66.xml"}}, {"value": "0", "module": "A1-A3"}, {"value": "0", "module": "A4"}, {"value": "0.65076", "module": "A5"}, {"value": "0", "module": "C1"}, {"value": "0", "module": "C2"}, {"value": "0", "module": "C3"}, {"value": "0", "module": "C4"}, {"value": "0", "module": "D"}]}, "resolvedFlowVersion": "38.00.000", "flowProperties": [], "typeOfFlow": "Other flow", "classification": {"classHierarchy": "Quantities / Environmental quantities / EPD EN 15804 / LCI indicators", "name": "GaBiCategories"}}]}, "LCIAResults": {"LCIAResult": [{"referenceToLCIAMethodDataSet": {"shortDescription": [{"value": "Globales Erwärmungspotenzial total (GWP-total)", "lang": "de"}, {"value": "Global Warming Potential total (GWP-total)", "lang": "en"}], "type": "LCIA method data set", "refObjectId": "6a37f984-a4b3-458a-a20a-64418c145fa2", "uri": "../lciamethods/6a37f984-a4b3-458a-a20a-64418c145fa2.xml"}, "other": {"anies": [{"name": "referenceToUnitGroupDataSet", "value": {"shortDescription": [{"value": "kg CO_(2)-Äq.", "lang": "de"}], "type": "unit group data set", "refObjectId": "1ebf3012-d0db-4de2-aefd-ef30cedb0be1", "uri": "../unitgroups/1ebf3012-d0db-4de2-aefd-ef30cedb0be1.xml"}}, {"value": "1.0786573466396", "module": "A1-A3"}, {"value": "0.0240670245179066", "module": "A4"}, {"value": "0.454674166430043", "module": "A5"}, {"value": "0", "module": "C1"}, {"value": "0.00206841805544456", "module": "C2"}, {"value": "0", "module": "C3"}, {"value": "0.00727657303219126", "module": "C4"}, {"value": "-0.0533412613712809", "module": "D"}]}}, {"referenceToLCIAMethodDataSet": {"shortDescription": [{"value": "Globales Erwärmungspotenzial fossil (GWP-fossil)", "lang": "de"}, {"value": "Global Warming Potential fossil fuels (GWP-fossil)", "lang": "en"}], "type": "LCIA method data set", "refObjectId": "5f635281-343e-44fb-83df-1971b155e6b6", "uri": "../lciamethods/5f635281-343e-44fb-83df-1971b155e6b6.xml"}, "other": {"anies": [{"name": "referenceToUnitGroupDataSet", "value": {"shortDescription": [{"value": "kg CO_(2)-Äq.", "lang": "de"}], "type": "unit group data set", "refObjectId": "1ebf3012-d0db-4de2-aefd-ef30cedb0be1", "uri": "../unitgroups/1ebf3012-d0db-4de2-aefd-ef30cedb0be1.xml"}}, {"value": "1.24358785917103", "module": "A1-A3"}, {"value": "0.0240722328496309", "module": "A4"}, {"value": "0.173697283613718", "module": "A5"}, {"value": "0", "module": "C1"}, {"value": "0.00206886568067423", "module": "C2"}, {"value": "0", "module": "C3"}, {"value": "0.0072759134243279", "module": "C4"}, {"value": "-0.0532477107245116", "module": "D"}]}}, {"referenceToLCIAMethodDataSet": {"shortDescription": [{"value": "Globales Erwärmungspotenzial biogen (GWP-biogenic)", "lang": "de"}, {"value": "Global Warming Potential biogenic (GWP-biogenic)", "lang": "en"}], "type": "LCIA method data set", "refObjectId": "2356e1ab-0185-4db5-86e5-16de51c7485c", "uri": "../lciamethods/2356e1ab-0185-4db5-86e5-16de51c7485c.xml"}, "other": {"anies": [{"name": "referenceToUnitGroupDataSet", "value": {"shortDescription": [{"value": "kg CO_(2)-Äq.", "lang": "de"}], "type": "unit group data set", "refObjectId": "1ebf3012-d0db-4de2-aefd-ef30cedb0be1", "uri": "../unitgroups/1ebf3012-d0db-4de2-aefd-ef30cedb0be1.xml"}}, {"value": "-0.165623089348367", "module": "A1-A3"}, {"value": "-6.74224989252569E-06", "module": "A4"}, {"value": "0.280962193311373", "module": "A5"}, {"value": "0", "module": "C1"}, {"value": "-5.7945640108702E-07", "module": "C2"}, {"value": "0", "module": "C3"}, {"value": "2.0942584916887E-07", "module": "C4"}, {"value": "-5.34392265256115E-05", "module": "D"}]}}, {"referenceToLCIAMethodDataSet": {"shortDescription": [{"value": "Globales Erwärmungspotenzial luluc (GWP-luluc)", "lang": "de"}, {"value": "Global Warming Potential luluc (GWP-luluc)", "lang": "en"}], "type": "LCIA method data set", "refObjectId": "4331bbdb-978a-490d-8707-eeb047f01a55", "uri": "../lciamethods/4331bbdb-978a-490d-8707-eeb047f01a55.xml"}, "other": {"anies": [{"name": "referenceToUnitGroupDataSet", "value": {"shortDescription": [{"value": "kg CO_(2)-Äq.", "lang": "de"}], "type": "unit group data set", "refObjectId": "1ebf3012-d0db-4de2-aefd-ef30cedb0be1", "uri": "../unitgroups/1ebf3012-d0db-4de2-aefd-ef30cedb0be1.xml"}}, {"value": "0.000692576816931104", "module": "A1-A3"}, {"value": "1.53391816824189E-06", "module": "A4"}, {"value": "1.46895049520375E-05", "module": "A5"}, {"value": "0", "module": "C1"}, {"value": "1.31831171419023E-07", "module": "C2"}, {"value": "0", "module": "C3"}, {"value": "4.50182014189431E-07", "module": "C4"}, {"value": "-4.01114202436531E-05", "module": "D"}]}}, {"referenceToLCIAMethodDataSet": {"shortDescription": [{"value": "Abbau Potential der stratosphärischen Ozonschicht (ODP)", "lang": "de"}, {"value": "Depletion potential of the stratospheric ozone layer (ODP)", "lang": "en"}], "type": "LCIA method data set", "refObjectId": "b5c629d6-def3-11e6-bf01-fe55135034f3", "uri": "../lciamethods/b5c629d6-def3-11e6-bf01-fe55135034f3.xml"}, "other": {"anies": [{"name": "referenceToUnitGroupDataSet", "value": {"shortDescription": [{"value": "kg CFC11-Äq.", "lang": "de"}], "type": "unit group data set", "refObjectId": "d9e957c9-7309-4474-bf3a-7777df6c4e5b", "uri": "../unitgroups/d9e957c9-7309-4474-bf3a-7777df6c4e5b.xml"}}, {"value": "1.34278028657245E-07", "module": "A1-A3"}, {"value": "1.22736300518367E-09", "module": "A4"}, {"value": "3.24192216040146E-09", "module": "A5"}, {"value": "0", "module": "C1"}, {"value": "1.0548457282776E-10", "module": "C2"}, {"value": "0", "module": "C3"}, {"value": "7.96286996758463E-10", "module": "C4"}, {"value": "-8.45383219306505E-09", "module": "D"}]}}, {"referenceToLCIAMethodDataSet": {"shortDescription": [{"value": "Versauerungspotenzial von Boden und Wasser (AP)", "lang": "de"}, {"value": "Acidification potential of land and water (AP)", "lang": "en"}], "type": "LCIA method data set", "refObjectId": "b5c611c6-def3-11e6-bf01-fe55135034f3", "uri": "../lciamethods/b5c611c6-def3-11e6-bf01-fe55135034f3.xml"}, "other": {"anies": [{"name": "referenceToUnitGroupDataSet", "value": {"shortDescription": [{"value": "mol H^(+)-Äq.", "lang": "de"}], "type": "unit group data set", "refObjectId": "42e089ac-92bf-4bf2-8ca1-5fc40d18f2ed", "uri": "../unitgroups/42e089ac-92bf-4bf2-8ca1-5fc40d18f2ed.xml"}}, {"value": "0.00964583388038749", "module": "A1-A3"}, {"value": "0.000171603760670719", "module": "A4"}, {"value": "0.000266248671595505", "module": "A5"}, {"value": "0", "module": "C1"}, {"value": "1.47483257304786E-05", "module": "C2"}, {"value": "0", "module": "C3"}, {"value": "5.7199852769202E-05", "module": "C4"}, {"value": "-6.78597281244011E-05", "module": "D"}]}}, {"referenceToLCIAMethodDataSet": {"shortDescription": [{"value": "Eutrophierungspotenzial Süßwasser (EP-freshwater)", "lang": "de"}, {"value": "Eutrophication potential aquatic freshwater (EP-freshwater)", "lang": "en"}], "type": "LCIA method data set", "refObjectId": "b53ec18f-7377-4ad3-86eb-cc3f4f276b2b", "uri": "../lciamethods/b53ec18f-7377-4ad3-86eb-cc3f4f276b2b.xml"}, "other": {"anies": [{"name": "referenceToUnitGroupDataSet", "value": {"shortDescription": [{"value": "kg PO_(4)-Äq.", "lang": "de"}], "type": "unit group data set", "refObjectId": "0429039d-a61d-4590-ba67-aa4a20a810a1", "uri": "../unitgroups/0429039d-a61d-4590-ba67-aa4a20a810a1.xml"}}, {"value": "4.27851660963969E-05", "module": "A1-A3"}, {"value": "3.25549241973268E-07", "module": "A4"}, {"value": "1.07396415119872E-06", "module": "A5"}, {"value": "0", "module": "C1"}, {"value": "2.79790270514242E-08", "module": "C2"}, {"value": "0", "module": "C3"}, {"value": "6.18738595647553E-08", "module": "C4"}, {"value": "-8.45133297022362E-07", "module": "D"}]}}, {"referenceToLCIAMethodDataSet": {"shortDescription": [{"value": "Eutrophierungspotenzial Salzwasser (EP-marine)", "lang": "de"}, {"value": "Eutrophication potential aquatic marine (EP-marine)", "lang": "en"}], "type": "LCIA method data set", "refObjectId": "b5c619fa-def3-11e6-bf01-fe55135034f3", "uri": "../lciamethods/b5c619fa-def3-11e6-bf01-fe55135034f3.xml"}, "other": {"anies": [{"name": "referenceToUnitGroupDataSet", "value": {"shortDescription": [{"value": "kg N-Äq.", "lang": "de"}], "type": "unit group data set", "refObjectId": "d05bb823-ecdf-4686-8c40-bf1d9257859f", "uri": "../unitgroups/d05bb823-ecdf-4686-8c40-bf1d9257859f.xml"}}, {"value": "0.000963234984030327", "module": "A1-A3"}, {"value": "7.3309145060782E-05", "module": "A4"}, {"value": "4.76813465173069E-05", "module": "A5"}, {"value": "0", "module": "C1"}, {"value": "6.30048634221922E-06", "module": "C2"}, {"value": "0", "module": "C3"}, {"value": "2.37825416008444E-05", "module": "C4"}, {"value": "-1.42019192317882E-05", "module": "D"}]}}, {"referenceToLCIAMethodDataSet": {"shortDescription": [{"value": "Eutrophierungspotenzial Land (EP-terrestrial)", "lang": "de"}, {"value": "Eutrophication potential terrestrial (EP-terrestrial)", "lang": "en"}], "type": "LCIA method data set", "refObjectId": "b5c614d2-def3-11e6-bf01-fe55135034f3", "uri": "../lciamethods/b5c614d2-def3-11e6-bf01-fe55135034f3.xml"}, "other": {"anies": [{"name": "referenceToUnitGroupDataSet", "value": {"shortDescription": [{"value": "mol N-Äq.", "lang": "de"}], "type": "unit group data set", "refObjectId": "71b4d617-0ec9-4d3f-b65e-e438940c2401", "uri": "../unitgroups/71b4d617-0ec9-4d3f-b65e-e438940c2401.xml"}}, {"value": "0.03704408110788", "module": "A1-A3"}, {"value": "0.000805773914700426", "module": "A4"}, {"value": "0.00106399394118087", "module": "A5"}, {"value": "0", "module": "C1"}, {"value": "6.9251490251009E-05", "module": "C2"}, {"value": "0", "module": "C3"}, {"value": "0.000261579455525485", "module": "C4"}, {"value": "-0.000156544780126823", "module": "D"}]}}, {"referenceToLCIAMethodDataSet": {"shortDescription": [{"value": "Bildungspotential für troposphärisches Ozon (POCP)", "lang": "de"}, {"value": "Formation potential of tropospheric ozone photochemical oxidants (POCP)", "lang": "en"}], "type": "LCIA method data set", "refObjectId": "b5c610fe-def3-11e6-bf01-fe55135034f3", "uri": "../lciamethods/b5c610fe-def3-11e6-bf01-fe55135034f3.xml"}, "other": {"anies": [{"name": "referenceToUnitGroupDataSet", "value": {"shortDescription": [{"value": "kg NMVOC-Äq.", "lang": "de"}], "type": "unit group data set", "refObjectId": "d27c25f8-fbc1-44c6-b47b-4adbae4199c6", "uri": "../unitgroups/d27c25f8-fbc1-44c6-b47b-4adbae4199c6.xml"}}, {"value": "0.00306990566341368", "module": "A1-A3"}, {"value": "0.000228375695062879", "module": "A4"}, {"value": "0.000155223225499469", "module": "A5"}, {"value": "0", "module": "C1"}, {"value": "1.96275368706795E-05", "module": "C2"}, {"value": "0", "module": "C3"}, {"value": "7.79052079309983E-05", "module": "C4"}, {"value": "-5.35726417208927E-05", "module": "D"}]}}, {"referenceToLCIAMethodDataSet": {"shortDescription": [{"value": "Potenzial für den abiotischen Abbau nicht fossiler Ressourcen (ADPE)", "lang": "de"}, {"value": "Abiotic depletion potential for non fossil resources (ADPE)", "lang": "en"}], "type": "LCIA method data set", "refObjectId": "b2ad6494-c78d-11e6-9d9d-cec0c932ce01", "uri": "../lciamethods/b2ad6494-c78d-11e6-9d9d-cec0c932ce01.xml"}, "other": {"anies": [{"name": "referenceToUnitGroupDataSet", "value": {"shortDescription": [{"value": "kg Sb-Äq.", "lang": "de"}], "type": "unit group data set", "refObjectId": "54ccd2d9-a32a-4fc2-923d-f2c8c93e89d4", "uri": "../unitgroups/54ccd2d9-a32a-4fc2-923d-f2c8c93e89d4.xml"}}, {"value": "1.83639882820279E-06", "module": "A1-A3"}, {"value": "5.59831009571141E-08", "module": "A4"}, {"value": "5.61997274272652E-08", "module": "A5"}, {"value": "0", "module": "C1"}, {"value": "4.81141558373011E-09", "module": "C2"}, {"value": "0", "module": "C3"}, {"value": "6.77967194807014E-09", "module": "C4"}, {"value": "-1.61937039521793E-08", "module": "D"}]}}, {"referenceToLCIAMethodDataSet": {"shortDescription": [{"value": "Potenzial für den abiotischen Abbau fossiler Brennstoffe (ADPF)", "lang": "de"}, {"value": "Abiotic depletion potential for fossil resources (ADPF)", "lang": "en"}], "type": "LCIA method data set", "refObjectId": "b2ad6110-c78d-11e6-9d9d-cec0c932ce01", "uri": "../lciamethods/b2ad6110-c78d-11e6-9d9d-cec0c932ce01.xml"}, "other": {"anies": [{"name": "referenceToUnitGroupDataSet", "value": {"shortDescription": [{"value": "MJ", "lang": "de"}], "type": "unit group data set", "refObjectId": "93a60a57-a3c8-11da-a746-0800200c9a66", "uri": "../unitgroups/93a60a57-a3c8-11da-a746-0800200c9a66.xml"}}, {"value": "27.0910677880111", "module": "A1-A3"}, {"value": "0.379614851401504", "module": "A4"}, {"value": "0.744290878434111", "module": "A5"}, {"value": "0", "module": "C1"}, {"value": "0.0326256456077302", "module": "C2"}, {"value": "0", "module": "C3"}, {"value": "0.183928692678052", "module": "C4"}, {"value": "-1.4579063562156", "module": "D"}]}}, {"referenceToLCIAMethodDataSet": {"shortDescription": [{"value": "Wassernutzung (WDP)", "lang": "de"}, {"value": "Water use (WDP)", "lang": "en"}], "type": "LCIA method data set", "refObjectId": "b2ad66ce-c78d-11e6-9d9d-cec0c932ce01", "uri": "../lciamethods/b2ad66ce-c78d-11e6-9d9d-cec0c932ce01.xml"}, "other": {"anies": [{"name": "referenceToUnitGroupDataSet", "value": {"shortDescription": [{"value": "m^(3) Welt-Äq. entzogen", "lang": "de"}], "type": "unit group data set", "refObjectId": "6ae2df01-888e-46c8-b17d-49fa3869b476", "uri": "../unitgroups/6ae2df01-888e-46c8-b17d-49fa3869b476.xml"}}, {"value": "654.901635169652", "module": "A1-A3"}, {"value": "1.14354727926095", "module": "A4"}, {"value": "13.7122087936046", "module": "A5"}, {"value": "0", "module": "C1"}, {"value": "0.0982811081576773", "module": "C2"}, {"value": "0", "module": "C3"}, {"value": "0.360233076266901", "module": "C4"}, {"value": "-39.2802866438817", "module": "D"}]}}, {"referenceToLCIAMethodDataSet": {"shortDescription": [{"value": "Auftreten von Krankheiten aufgrund von Feinstaubemissionen (PM)", "lang": "de"}, {"value": "Incidence of disease due to PM emissions (PM)", "lang": "en"}], "type": "LCIA method data set", "refObjectId": "b5c602c6-def3-11e6-bf01-fe55135034f3", "uri": "../lciamethods/b5c602c6-def3-11e6-bf01-fe55135034f3.xml"}, "other": {"anies": [{"name": "referenceToUnitGroupDataSet", "value": {"shortDescription": [{"value": "Krankheitsfälle", "lang": "de"}], "type": "unit group data set", "refObjectId": "3883559b-648f-4afc-8ba2-0bd24f3affa3", "uri": "../unitgroups/3883559b-648f-4afc-8ba2-0bd24f3affa3.xml"}}, {"value": "7.36623259670058E-08", "module": "A1-A3"}, {"value": "1.82793163691535E-09", "module": "A4"}, {"value": "2.1675220095667E-09", "module": "A5"}, {"value": "3.9591E-09", "module": "C1"}, {"value": "1.57099885742041E-10", "module": "C2"}, {"value": "0", "module": "C3"}, {"value": "1.07236720049706E-09", "module": "C4"}, {"value": "-2.61556525775041E-10", "module": "D"}]}}, {"referenceToLCIAMethodDataSet": {"shortDescription": [{"value": "Wirkung durch Exposition des Menschen mit U235 (IR)", "lang": "de"}, {"value": "Human exposure efficiency relative to U235 (IR)", "lang": "en"}], "type": "LCIA method data set", "refObjectId": "b5c632be-def3-11e6-bf01-fe55135034f3", "uri": "../lciamethods/b5c632be-def3-11e6-bf01-fe55135034f3.xml"}, "other": {"anies": [{"name": "referenceToUnitGroupDataSet", "value": {"shortDescription": [{"value": "kBq U235-Äq.", "lang": "de"}], "type": "unit group data set", "refObjectId": "456b05bf-1415-44a9-9993-02452f554c09", "uri": "../unitgroups/456b05bf-1415-44a9-9993-02452f554c09.xml"}}, {"value": "0.403321377498274", "module": "A1-A3"}, {"value": "0.000677515602897196", "module": "A4"}, {"value": "0.00840920763520414", "module": "A5"}, {"value": "0", "module": "C1"}, {"value": "5.822844884025E-05", "module": "C2"}, {"value": "0", "module": "C3"}, {"value": "0.000211245437180671", "module": "C4"}, {"value": "-0.0244300974601256", "module": "D"}]}}, {"referenceToLCIAMethodDataSet": {"shortDescription": [{"value": "Toxizitätsvergleichseinheit für Ökosysteme (ETP-fw)", "lang": "de"}, {"value": "Comparative toxic unit for ecosystems (ETP-fw)", "lang": "en"}], "type": "LCIA method data set", "refObjectId": "ee1082d1-b0f7-43ca-a1f0-21e2a4a74511", "uri": "../lciamethods/ee1082d1-b0f7-43ca-a1f0-21e2a4a74511.xml"}, "other": {"anies": [{"name": "referenceToUnitGroupDataSet", "value": {"shortDescription": [{"value": "CTUe", "lang": "de"}], "type": "unit group data set", "refObjectId": "aa959ded-f1eb-4efb-9c5c-2d60be36b3e6", "uri": "../unitgroups/aa959ded-f1eb-4efb-9c5c-2d60be36b3e6.xml"}}, {"value": "14.3593418739381", "module": "A1-A3"}, {"value": "0.168172470092625", "module": "A4"}, {"value": "0.423621016875834", "module": "A5"}, {"value": "0", "module": "C1"}, {"value": "0.0144534266506225", "module": "C2"}, {"value": "0", "module": "C3"}, {"value": "0.0614294250922464", "module": "C4"}, {"value": "-0.214049056521156", "module": "D"}]}}, {"referenceToLCIAMethodDataSet": {"shortDescription": [{"value": "Toxizitätsvergleichseinheit für Menschen (krebserregend) (HTP-c)", "lang": "de"}, {"value": "Comparative toxic unit for humans (carcinogenic) (HTP-c)", "lang": "en"}], "type": "LCIA method data set", "refObjectId": "2299222a-bbd8-474f-9d4f-4dd1f18aea7c", "uri": "../lciamethods/2299222a-bbd8-474f-9d4f-4dd1f18aea7c.xml"}, "other": {"anies": [{"name": "referenceToUnitGroupDataSet", "value": {"shortDescription": [{"value": "CTUh", "lang": "de"}], "type": "unit group data set", "refObjectId": "d4c9523e-2d7e-49fd-8469-998f547d3a70", "uri": "../unitgroups/d4c9523e-2d7e-49fd-8469-998f547d3a70.xml"}}, {"value": "2.50586241457099E-10", "module": "A1-A3"}, {"value": "1.43871282702882E-11", "module": "A4"}, {"value": "5.00132166793765E-11", "module": "A5"}, {"value": "0", "module": "C1"}, {"value": "1.23648836847777E-12", "module": "C2"}, {"value": "0", "module": "C3"}, {"value": "2.53260324792916E-12", "module": "C4"}, {"value": "-5.69912082064032E-12", "module": "D"}]}}, {"referenceToLCIAMethodDataSet": {"shortDescription": [{"value": "Toxizitätsvergleichseinheit für Menschen (nicht krebserregend) (HTP-nc)", "lang": "de"}, {"value": "Comparative toxic unit for humans (noncarcinogenic) (HTP-nc)", "lang": "en"}], "type": "LCIA method data set", "refObjectId": "3af763a5-b7a1-48c9-9cee-1f223481fcef", "uri": "../lciamethods/3af763a5-b7a1-48c9-9cee-1f223481fcef.xml"}, "other": {"anies": [{"name": "referenceToUnitGroupDataSet", "value": {"shortDescription": [{"value": "CTUh", "lang": "de"}], "type": "unit group data set", "refObjectId": "d4c9523e-2d7e-49fd-8469-998f547d3a70", "uri": "../unitgroups/d4c9523e-2d7e-49fd-8469-998f547d3a70.xml"}}, {"value": "6.70724350848434E-09", "module": "A1-A3"}, {"value": "2.65631514487061E-10", "module": "A4"}, {"value": "8.03739879253622E-10", "module": "A5"}, {"value": "0", "module": "C1"}, {"value": "2.28294536473058E-11", "module": "C2"}, {"value": "0", "module": "C3"}, {"value": "6.48723942853533E-11", "module": "C4"}, {"value": "-1.15479723747334E-10", "module": "D"}]}}, {"referenceToLCIAMethodDataSet": {"shortDescription": [{"value": "Bodenqualitätsindex (SQP)", "lang": "de"}, {"value": "Soil quality index (SQP)", "lang": "en"}], "type": "LCIA method data set", "refObjectId": "b2ad6890-c78d-11e6-9d9d-cec0c932ce01", "uri": "../lciamethods/b2ad6890-c78d-11e6-9d9d-cec0c932ce01.xml"}, "other": {"anies": [{"name": "referenceToUnitGroupDataSet", "value": {"shortDescription": [{"value": "SQP", "lang": "de"}], "type": "unit group data set", "refObjectId": "f130951c-e67f-4f7f-8dd4-665de3974e18", "uri": "../unitgroups/f130951c-e67f-4f7f-8dd4-665de3974e18.xml"}}, {"value": "1.3604460089179", "module": "A1-A3"}, {"value": "0.0482548792707574", "module": "A4"}, {"value": "0.0417515123691329", "module": "A5"}, {"value": "0", "module": "C1"}, {"value": "0.00414722075313753", "module": "C2"}, {"value": "0", "module": "C3"}, {"value": "0.322854299211136", "module": "C4"}, {"value": "-0.0111645586868847", "module": "D"}]}}]}, "otherAttributes": {"{http://www.indata.network/EPD/2019}epd-version": "1.2"}, "version": "1.1", "locations": "../ILCDLocations.xml"}