{"processInformation": {"dataSetInformation": {"UUID": "0144d30d-e4d7-4c05-a4c5-282772589893", "name": {"baseName": [{"value": "Putzmörtel-Normalputz/Edelputz mit besonderen Eigenschaften", "lang": "de"}, {"value": "Rendering Mortar - Normal Render/Finishing Render With Special Properties", "lang": "en"}], "functionalUnitFlowProperties": [{"lang": "de"}]}, "classificationInformation": {"classification": [{"class": [{"value": "Mineralische Baustoffe", "level": 0, "classId": "1"}, {"value": "Mörtel und Beton", "level": 1, "classId": "1.4"}, {"value": "Putz und Putzmörtel", "level": 2, "classId": "1.4.04"}], "name": "OEKOBAU.DAT"}, {"class": [{"value": "02 Bauprodukte", "level": 0}, {"value": "Mauerwerk und Mörtel", "level": 1}, {"value": "Mineralische Werkmörtel", "level": 2}], "name": "IBUCategories"}]}, "generalComment": [{"value": "Mineralische Werkmrtel sind Mrtel, deren Bestandteile im Werk und nicht auf der Baustelle gemischt werden. Sie werden in Abhngigkeit von der Art der Verwendung in die drei Werkmrtelarten Mauermrtel, Putzmrtel und Estrichmrtel unterteilt.\nMineralische Putzmrtel sind Gemische aus einem oder mehreren anorganischen Bindemitteln, Zuschlgen, Wasser und ggf. Zusatzstoffen bzw. Zusatzmitteln zur Herstellung von Auen- oder Innenputzen. Putzmrtel werden an Wnden und Decken je nach Erfordernis ein- oder mehrlagig aufgetragen. Neben der sthetischen Gestaltung der Oberflche dienen sie als Auenputze der Abhaltung der Witterungseinflsse und als Innenputze der ebenflchigen Unterlage von Anstrichen und Tapeten. Bei Stahlbetondecken und -treppen dienen Putze auch dem Brandschutz, durch Zugabe poriger Zuschlge auch dem Wrmeschutz. Abhngig von den technischen Daten, den eingesetzten Grund- und Hilfsstoffen und der praktischen Anwendung werden Putzmrtel in die Produktgruppen Normalputz/Edelputz, Normalputz/Edelputz mit besonderen Eigenschaften, Leichtputz, Armierungsputz und Wrmedmmputz mit besonders hohem Anteil an Leichtzuschlgen unterteilt.", "lang": "de"}]}, "quantitativeReference": {"referenceToReferenceFlow": [0]}, "time": {"referenceYear": 2024, "dataSetValidUntil": 2029, "other": {"anies": [{"name": "publicationDateOfEPD", "value": 1710201600000}]}}, "geography": {"locationOfOperationSupplyOrProduction": {"location": "DE"}}, "technology": {"technologyDescriptionAndIncludedProcesses": [{"value": "In der Graphik ist der Herstellungsprozess dargestellt. Mineralische Putzmörtel werden in Mischwerken in folgenden Arbeitsschritten hergestellt: Füllen der Vorrats- bzw. Wägebehälter, Förderung der Einsatzstoffe/des Mischgutes in den Mischer, Mischen, Förderung des Fertigproduktes, Verpackung, Verladung des Fertigproduktes und Auslieferung.Die Rohstoffe – Sand, Bindemittel, Leichtzuschläge, Hilfsstoffe, Zusatzmittel und -stoffe (siehe Grundstoffe) – werden im Herstellwerk in Silos gelagert. Aus den Silos werden die Rohstoffe entsprechend der jeweiligen Rezeptur gravimetrisch dosiert und intensiv miteinander vermischt. Anschließend wird das Mischgut abgepackt und als Werk-Trockenmörtel trocken in Gebinden oder Silos ausgeliefert. Graphik 1: Herstellungsprozess (grün: Input; blau: Einheitsprozess) \nDeklarierte Einheit: \nDiese Deklaration bezieht sich auf die Herstellung von einem Kilogramm typischer Putzmrtel der Produktgruppe Normalputz/Edelputz mit besonderen Eigenschaften. Es werden ausschlielich Trockenmrtel betrachtet.", "lang": "de"}, {"value": "Mineral rendering mortars are produced in mixing plants in the following work steps: - Filling the storage or weighing containers, - Feeding the ingredients/mixed material into the mixer, - Mixing, - Conveying of the finished product, - Packaging, - Loading of the finished product and delivery. The raw materials - sand, binders, lightweight aggregates, auxiliary materials, admixtures and additives - are stored in silos at the manufacturing plant. From the silos, the raw materials are gravimetrically dosed according to the respective recipe and intensively mixed with each other. The mix is then packaged and delivered dry in containers or silos as factory dry mortar. Technical Data: Compressive strength according to EN 1015-11 ≤ 15 N/mm2 Thermal conductivity according to EN 1745 lambda10,dry,mat / P = 50 %: 0.39 - 0.82 W/(mK) Thermal conductivity according to EN 1745 lambda10,dry,mat / P = 90 %: 0.43 - 0.89 W/(mK) Water vapour permeability according to EN 1015-19: 15/35 - Dry bulk density according to EN 1015-10: 1300 - 1800 kg/m³ Capillary water absorption according to EN 1015-18: not specified Sound absorption coefficient, adhesive shear strength, adhesive tensile strength and flexural tensile strength are not relevant. Declared Unit: 1 kg rendering mortar as a mineral factory-made mortar, product group normal render/finishing render with special properties with a dry bulk density > 1300 kg/m³ and < 1800 kg/m³.", "lang": "en"}], "technologicalApplicability": [{"value": "Im Werk hergestellte Putzmrtel zur Verwendung als Unterputz bzw. Oberputz auf Wnden, Decken, Pfeilern und Trennwnden von Baukrpern, die den geltenden Normen entsprechen oder auf hnlichen Putzgrnden (z. B. bei Bestandsgebuden).\nNormalputz zur Herstellung von Innen- und Auenputz mit besonderen Eigenschaften (z.B. Weigrad, Oberflchengte oder Elastizitt).", "lang": "de"}, {"value": "Rendering mortar produced in the factory for use as a base coat or finishing render on walls, ceilings, pillars and partitions of building structures that comply with the applicable standards or on similar rendering substrates (e.g. in existing buildings). Normal render for the production of interior and exterior render with special properties (e.g. whiteness, surface quality or elasticity).", "lang": "en"}]}}, "modellingAndValidation": {"LCIMethodAndAllocation": {"typeOfDataSet": "EPD", "referenceToLCAMethodDetails": [{"shortDescription": [{"value": "Mineralische Werkmörtel.pdf", "lang": "de"}], "type": "source data set", "refObjectId": "e4791a54-36ad-4a7c-a88c-151250a58bbd"}], "other": {"anies": [{"name": "subType", "value": "template dataset"}]}}, "dataSourcesTreatmentAndRepresentativeness": {"referenceToDataSource": [{"shortDescription": [{"value": "GaBi Database (all versions)", "lang": "de"}], "type": "source data set", "refObjectId": "28d74cc0-db8b-4d7e-bc44-5f6d56ce0c4a"}, {"shortDescription": [{"value": "GaBi Database Edition 2022, CUP 2022.02", "lang": "de"}], "type": "source data set", "refObjectId": "94f442cb-662e-43ea-a792-4b0a35132e93"}], "useAdviceForDataSet": [{"value": "Gültigkeitsbereich: \nBei diesem Dokument handelt es sich um eine Muster-EPD, bei der fr die Berechnung der kobilanz das Produkt einer Gruppe ausgewhlt wurde, welches die hchsten Umweltlasten dieser Gruppe aufweist. Sie gilt ausschlielich fr Putzmrtel-Normalputz/Edelputz mit besonderen Eigenschaften als mineralische Werkmrtel fr Verbandsmitglieder; diese knnen der Verbandswebsite entnommen werden. Bei den Zahlenangaben, zum Beispiel fr bautechnische Daten oder Konzentrationsangaben, handelt es sich um durchschnittliche praxisbliche Werte fr diese Produktgruppe. \nSystemgrenze: \nDie Lebenszyklusanalyse der untersuchten Produkte umfasst die Produktion des Mrtels einschlielich der Rohstoffgewinnung und Energietrgerbereitstellung bis zum fertig verpackten Produkt (Modul A1–A3), den Einbau des Produktes inkl. Transport zur Baustelle (Modul A4–A5), die Nutzungsphase (Modul B1) sowie die Entsorgung des Mrtels (Modul C1–C4). Fr Siloware werden die anteiligen Aufwendungen fr den Transport und die Herstellung des Silos bercksichtigt. Gutschriften fr die Verpackung einschlielich Energierckgewinnung (Modul D) gehen ebenfalls in die kobilanz ein.", "lang": "de"}], "other": {"anies": [{"name": "referenceToOriginalEPD", "value": {"shortDescription": {"value": "Putzmörtel-Normalputz/Edelputz mit besonderen Eigenschaften.pdf", "defaultValue": "Putzmörtel-Normalputz/Edelputz mit besonderen Eigenschaften.pdf", "lstrings": [{"lang": "de", "value": "Putzmörtel-Normalputz/Edelputz mit besonderen Eigenschaften.pdf"}]}, "type": "source data set", "uuid": {"uuid": "e0681cb9-ba29-40e8-815e-0f4827e6c267"}, "refObjectId": "e0681cb9-ba29-40e8-815e-0f4827e6c267", "resourceURLs": ["https://oekobaudat.de/OEKOBAU.DAT/resource/sources/e0681cb9-ba29-40e8-815e-0f4827e6c267/Putzmoertel-NormalputzEdelputz_mit_besonderen_Eigenschaften_24252.pdf?version=00.02.000"]}}]}}, "validation": {"review": [{"referenceToNameOfReviewerAndInstitution": [{"shortDescription": [{"value": "Institut Bauen und Umwelt e. V.", "lang": "de"}], "type": "contact data set", "refObjectId": "d111dbec-b024-4be5-86c5-752d6eb2cf95", "uri": "../contacts/d111dbec-b024-4be5-86c5-752d6eb2cf95.xml"}], "type": "Accredited third party review"}]}, "complianceDeclarations": {"compliance": [{"referenceToComplianceSystem": {"shortDescription": [{"value": "DIN EN 15804+A2", "lang": "de"}], "type": "source data set", "refObjectId": "c0016b33-8cf7-415c-ac6e-deba0d21440d", "uri": "../sources/c0016b33-8cf7-415c-ac6e-deba0d21440d.xml"}}, {"referenceToComplianceSystem": {"shortDescription": [{"value": "ISO 14025", "lang": "de"}], "type": "source data set", "refObjectId": "4f2eb655-6e44-4874-a95a-e28f5442cd4d", "uri": "../sources/4f2eb655-6e44-4874-a95a-e28f5442cd4d.xml"}}]}}, "administrativeInformation": {"commissionerAndGoal": {"referenceToCommissioner": [{"shortDescription": [{"value": "Verband für Dämmsysteme, Putz und Mörtel e.V. (VDPM)", "lang": "de"}], "type": "contact data set", "refObjectId": "d6bb6100-c0b6-4892-9bb7-20127d85b172", "uri": "../contacts/d6bb6100-c0b6-4892-9bb7-20127d85b172.xml"}]}, "dataGenerator": {"referenceToPersonOrEntityGeneratingTheDataSet": [{"shortDescription": [{"value": "Sphera Solutions GmbH", "lang": "de"}], "type": "contact data set", "refObjectId": "623edf96-39d1-4e6f-9892-674c7228546b", "uri": "../contacts/623edf96-39d1-4e6f-9892-674c7228546b.xml"}]}, "dataEntryBy": {"timeStamp": 1710201600000, "referenceToDataSetFormat": [{"shortDescription": [{"value": "ILCD Format", "lang": "de"}], "type": "source data set", "refObjectId": "a97a0155-0234-4b87-b4ce-a45da52f2a40", "uri": "../sources/a97a0155-0234-4b87-b4ce-a45da52f2a40.xml"}, {"shortDescription": [{"value": "EPD-Datenformaterweiterungen v1.2", "lang": "de"}, {"value": "EPD Data Format Extensions v1.2", "lang": "en"}], "type": "source data set", "refObjectId": "a29449fd-aa2f-4de8-b5d7-4b06b43c6fde", "uri": "../sources/a29449fd-aa2f-4de8-b5d7-4b06b43c6fde.xml"}]}, "publicationAndOwnership": {"dataSetVersion": "00.01.000", "referenceToPrecedingDataSetVersion": [{"shortDescription": [{"value": "Putzmörtel-Normalputz/Edelputz mit besonderen Eigenschaften", "lang": "de"}], "type": "process data set", "refObjectId": "d154c187-5117-46e1-9b78-a3a9a39a3abf", "uri": "../processes/d154c187-5117-46e1-9b78-a3a9a39a3abf.xml"}], "referenceToRegistrationAuthority": {"shortDescription": [{"value": "Institut Bauen und Umwelt e. V.", "lang": "de"}], "type": "contact data set", "refObjectId": "d111dbec-b024-4be5-86c5-752d6eb2cf95", "uri": "../contacts/d111dbec-b024-4be5-86c5-752d6eb2cf95.xml"}, "registrationNumber": "EPD-VDP-20230399-IBO1-DE", "referenceToOwnershipOfDataSet": {"shortDescription": [{"value": "Verband für Dämmsysteme, Putz und Mörtel e.V. (VDPM)", "lang": "de"}], "type": "contact data set", "refObjectId": "d6bb6100-c0b6-4892-9bb7-20127d85b172", "uri": "../contacts/d6bb6100-c0b6-4892-9bb7-20127d85b172.xml"}, "copyright": true, "licenseType": "Free of charge for all users and uses", "accessRestrictions": [{"value": "None", "lang": "en"}], "other": {"anies": [{"name": "referenceToPublisher", "value": {"shortDescription": [{"value": "Institut Bauen und Umwelt e. V.", "lang": "de"}], "type": "contact data set", "refObjectId": "d111dbec-b024-4be5-86c5-752d6eb2cf95", "uri": "../contacts/d111dbec-b024-4be5-86c5-752d6eb2cf95.xml"}}]}}}, "exchanges": {"exchange": [{"dataSetInternalID": 0, "referenceToFlowDataSet": {"shortDescription": [{"value": "1 kg Putzmörtel-Normalputz / Edelputz mit besonderen Eigenschaften (1 kg Putzmörtel-Normalputz / Edelputz mit besonderen Eigenschaften)", "lang": "de"}], "type": "flow data set", "refObjectId": "d7c6306c-da73-742d-afda-542390fec649", "uri": "../flows/d7c6306c-da73-742d-afda-542390fec649.xml"}, "meanAmount": 1.0, "referencesToDataSource": {}, "referenceFlow": true, "resolvedFlowVersion": "00.01.000", "resultingflowAmount": 1.0, "flowProperties": [{"name": [{"lang": "en", "value": "Mass"}, {"lang": "de", "value": "Masse"}], "uuid": "93a60a56-a3c8-11da-a746-0800200b9a66", "referenceFlowProperty": true, "meanValue": 1.0, "referenceUnit": "kg", "unitGroupUUID": "ad38d542-3fe9-439d-9b95-2f5f7752acaf"}], "materialProperties": [{"name": "gross density", "value": "1550.0", "unit": "kg/m^3", "unitDescription": "kilograms per cubic metre"}], "typeOfFlow": "Product flow", "classification": {"classHierarchy": "Mineralische Baustoffe / Mörtel und Beton / Putz und Putzmörtel", "name": "OEKOBAU.DAT"}}, {"dataSetInternalID": 1, "referenceToFlowDataSet": {"shortDescription": [{"value": "Erneuerbare Primärenergie als Energieträger (PERE)", "lang": "de"}, {"value": "Renewable primary energy as energy carrier (PERE)", "lang": "en"}], "type": "flow data set", "refObjectId": "20f32be5-0398-4288-9b6d-accddd195317", "uri": "../flows/20f32be5-0398-4288-9b6d-accddd195317.xml"}, "exchange direction": "INPUT", "other": {"anies": [{"name": "referenceToUnitGroupDataSet", "value": {"shortDescription": [{"value": "MJ", "lang": "de"}], "type": "unit group data set", "refObjectId": "93a60a57-a3c8-11da-a746-0800200c9a66", "uri": "../unitgroups/93a60a57-a3c8-11da-a746-0800200c9a66.xml"}}, {"value": "0.743", "module": "A1-A3"}, {"value": "0.00878", "module": "A4"}, {"value": "0.33", "module": "A5"}, {"value": "0", "module": "B1"}, {"value": "0.00025", "module": "C1"}, {"value": "0.00455", "module": "C2"}, {"value": "0", "module": "C3"}, {"value": "0.0312", "module": "C4"}, {"value": "-0.0749", "module": "D"}]}, "resolvedFlowVersion": "38.00.000", "flowProperties": [], "typeOfFlow": "Other flow", "classification": {"classHierarchy": "Quantities", "name": "GaBiCategories"}}, {"dataSetInternalID": 2, "referenceToFlowDataSet": {"shortDescription": [{"value": "Erneuerbare Primärenergie zur stofflichen Nutzung (PERM)", "lang": "de"}, {"value": "Renewable primary energy resources as material utilization (PERM)", "lang": "en"}], "type": "flow data set", "refObjectId": "fb3ec0de-548d-4508-aea5-00b73bf6f702", "uri": "../flows/fb3ec0de-548d-4508-aea5-00b73bf6f702.xml"}, "exchange direction": "INPUT", "other": {"anies": [{"name": "referenceToUnitGroupDataSet", "value": {"shortDescription": [{"value": "MJ", "lang": "de"}], "type": "unit group data set", "refObjectId": "93a60a57-a3c8-11da-a746-0800200c9a66", "uri": "../unitgroups/93a60a57-a3c8-11da-a746-0800200c9a66.xml"}}, {"value": "0.286", "module": "A1-A3"}, {"value": "0", "module": "A4"}, {"value": "-0.286", "module": "A5"}, {"value": "0", "module": "B1"}, {"value": "0", "module": "C1"}, {"value": "0", "module": "C2"}, {"value": "0", "module": "C3"}, {"value": "0", "module": "C4"}, {"value": "0", "module": "D"}]}, "resolvedFlowVersion": "38.00.000", "flowProperties": [], "typeOfFlow": "Other flow", "classification": {"classHierarchy": "Quantities", "name": "GaBiCategories"}}, {"dataSetInternalID": 3, "referenceToFlowDataSet": {"shortDescription": [{"value": "Total erneuerbare Primärenergie (PERT)", "lang": "de"}, {"value": "Total use of renewable primary energy resources (PERT)", "lang": "en"}], "type": "flow data set", "refObjectId": "53f97275-fa8a-4cdd-9024-65936002acd0", "uri": "../flows/53f97275-fa8a-4cdd-9024-65936002acd0.xml"}, "exchange direction": "INPUT", "other": {"anies": [{"name": "referenceToUnitGroupDataSet", "value": {"shortDescription": [{"value": "MJ", "lang": "de"}], "type": "unit group data set", "refObjectId": "93a60a57-a3c8-11da-a746-0800200c9a66", "uri": "../unitgroups/93a60a57-a3c8-11da-a746-0800200c9a66.xml"}}, {"value": "1.029", "module": "A1-A3"}, {"value": "0.00878", "module": "A4"}, {"value": "0.044", "module": "A5"}, {"value": "0", "module": "B1"}, {"value": "0.00025", "module": "C1"}, {"value": "0.00455", "module": "C2"}, {"value": "0", "module": "C3"}, {"value": "0.0312", "module": "C4"}, {"value": "-0.0749", "module": "D"}]}, "resolvedFlowVersion": "38.00.000", "flowProperties": [], "typeOfFlow": "Other flow", "classification": {"classHierarchy": "Quantities / Environmental quantities / EPD EN 15804 / LCI indicators", "name": "GaBiCategories"}}, {"dataSetInternalID": 4, "referenceToFlowDataSet": {"shortDescription": [{"value": "Nicht-erneuerbare Primärenergie als Energieträger (PENRE)", "lang": "de"}, {"value": "Non renewable primary energy as energy carrier (PENRE)", "lang": "en"}], "type": "flow data set", "refObjectId": "ac857178-2b45-46ec-892a-a9a4332f0372", "uri": "../flows/ac857178-2b45-46ec-892a-a9a4332f0372.xml"}, "exchange direction": "INPUT", "other": {"anies": [{"name": "referenceToUnitGroupDataSet", "value": {"shortDescription": [{"value": "MJ", "lang": "de"}], "type": "unit group data set", "refObjectId": "93a60a57-a3c8-11da-a746-0800200c9a66", "uri": "../unitgroups/93a60a57-a3c8-11da-a746-0800200c9a66.xml"}}, {"value": "3.208", "module": "A1-A3"}, {"value": "0.148", "module": "A4"}, {"value": "0.0509", "module": "A5"}, {"value": "0", "module": "B1"}, {"value": "0.00381", "module": "C1"}, {"value": "0.0767", "module": "C2"}, {"value": "0", "module": "C3"}, {"value": "0.207", "module": "C4"}, {"value": "-0.233", "module": "D"}]}, "resolvedFlowVersion": "38.00.000", "flowProperties": [], "typeOfFlow": "Other flow", "classification": {"classHierarchy": "Quantities", "name": "GaBiCategories"}}, {"dataSetInternalID": 5, "referenceToFlowDataSet": {"shortDescription": [{"value": "Nicht-erneuerbare Primärenergie zur stofflichen Nutzung (PENRM)", "lang": "de"}, {"value": "Non renewable primary energy as material utilization (PENRM)", "lang": "en"}], "type": "flow data set", "refObjectId": "1421caa0-679d-4bf4-b282-0eb850ccae27", "uri": "../flows/1421caa0-679d-4bf4-b282-0eb850ccae27.xml"}, "exchange direction": "INPUT", "other": {"anies": [{"name": "referenceToUnitGroupDataSet", "value": {"shortDescription": [{"value": "MJ", "lang": "de"}], "type": "unit group data set", "refObjectId": "93a60a57-a3c8-11da-a746-0800200c9a66", "uri": "../unitgroups/93a60a57-a3c8-11da-a746-0800200c9a66.xml"}}, {"value": "0.037", "module": "A1-A3"}, {"value": "0", "module": "A4"}, {"value": "-0.037", "module": "A5"}, {"value": "0", "module": "B1"}, {"value": "0", "module": "C1"}, {"value": "0", "module": "C2"}, {"value": "0", "module": "C3"}, {"value": "0", "module": "C4"}, {"value": "0", "module": "D"}]}, "resolvedFlowVersion": "38.00.000", "flowProperties": [], "typeOfFlow": "Other flow", "classification": {"classHierarchy": "Quantities", "name": "GaBiCategories"}}, {"dataSetInternalID": 6, "referenceToFlowDataSet": {"shortDescription": [{"value": "Total nicht erneuerbare Primärenergie (PENRT)", "lang": "de"}, {"value": "Total use of non renewable primary energy resources (PENRT)", "lang": "en"}], "type": "flow data set", "refObjectId": "06159210-646b-4c8d-8583-da9b3b95a6c1", "uri": "../flows/06159210-646b-4c8d-8583-da9b3b95a6c1.xml"}, "exchange direction": "INPUT", "other": {"anies": [{"name": "referenceToUnitGroupDataSet", "value": {"shortDescription": [{"value": "MJ", "lang": "de"}], "type": "unit group data set", "refObjectId": "93a60a57-a3c8-11da-a746-0800200c9a66", "uri": "../unitgroups/93a60a57-a3c8-11da-a746-0800200c9a66.xml"}}, {"value": "3.245", "module": "A1-A3"}, {"value": "0.148", "module": "A4"}, {"value": "0.0139", "module": "A5"}, {"value": "0", "module": "B1"}, {"value": "0.00381", "module": "C1"}, {"value": "0.0767", "module": "C2"}, {"value": "0", "module": "C3"}, {"value": "0.207", "module": "C4"}, {"value": "-0.233", "module": "D"}]}, "resolvedFlowVersion": "38.00.000", "flowProperties": [], "typeOfFlow": "Other flow", "classification": {"classHierarchy": "Quantities / Environmental quantities / EPD EN 15804 / LCI indicators", "name": "GaBiCategories"}}, {"dataSetInternalID": 7, "referenceToFlowDataSet": {"shortDescription": [{"value": "Einsatz von Sekundärstoffen (SM)", "lang": "de"}, {"value": "Use of secondary material (SM)", "lang": "en"}], "type": "flow data set", "refObjectId": "c6a1f35f-2d09-4f54-8dfb-97e502e1ce92", "uri": "../flows/c6a1f35f-2d09-4f54-8dfb-97e502e1ce92.xml"}, "exchange direction": "INPUT", "other": {"anies": [{"name": "referenceToUnitGroupDataSet", "value": {"shortDescription": [{"value": "kg", "lang": "de"}], "type": "unit group data set", "refObjectId": "ad38d542-3fe9-439d-9b95-2f5f7752acaf", "uri": "../unitgroups/ad38d542-3fe9-439d-9b95-2f5f7752acaf.xml"}}, {"value": "0", "module": "A1-A3"}, {"value": "0", "module": "A4"}, {"value": "0", "module": "A5"}, {"value": "0", "module": "B1"}, {"value": "0", "module": "C1"}, {"value": "0", "module": "C2"}, {"value": "0", "module": "C3"}, {"value": "0", "module": "C4"}, {"value": "0", "module": "D"}]}, "resolvedFlowVersion": "38.00.000", "flowProperties": [], "typeOfFlow": "Other flow", "classification": {"classHierarchy": "Quantities / Environmental quantities / EPD EN 15804 / LCI indicators", "name": "GaBiCategories"}}, {"dataSetInternalID": 8, "referenceToFlowDataSet": {"shortDescription": [{"value": "Erneuerbare Sekundärbrennstoffe (RSF)", "lang": "de"}, {"value": "Use of renewable secondary fuels (RSF)", "lang": "en"}], "type": "flow data set", "refObjectId": "64333088-a55f-4aa2-9a31-c10b07816787", "uri": "../flows/64333088-a55f-4aa2-9a31-c10b07816787.xml"}, "exchange direction": "INPUT", "other": {"anies": [{"name": "referenceToUnitGroupDataSet", "value": {"shortDescription": [{"value": "MJ", "lang": "de"}], "type": "unit group data set", "refObjectId": "93a60a57-a3c8-11da-a746-0800200c9a66", "uri": "../unitgroups/93a60a57-a3c8-11da-a746-0800200c9a66.xml"}}, {"value": "0", "module": "A1-A3"}, {"value": "0", "module": "A4"}, {"value": "0", "module": "A5"}, {"value": "0", "module": "B1"}, {"value": "0", "module": "C1"}, {"value": "0", "module": "C2"}, {"value": "0", "module": "C3"}, {"value": "0", "module": "C4"}, {"value": "0", "module": "D"}]}, "resolvedFlowVersion": "38.00.000", "flowProperties": [], "typeOfFlow": "Other flow", "classification": {"classHierarchy": "Quantities / Environmental quantities / EPD EN 15804 / LCI indicators", "name": "GaBiCategories"}}, {"dataSetInternalID": 9, "referenceToFlowDataSet": {"shortDescription": [{"value": "Nicht erneuerbare Sekundärbrennstoffe (NRSF)", "lang": "de"}, {"value": "Use of non renewable secondary fuels (NRSF)", "lang": "en"}], "type": "flow data set", "refObjectId": "89def144-d39a-4287-b86f-efde453ddcb2", "uri": "../flows/89def144-d39a-4287-b86f-efde453ddcb2.xml"}, "exchange direction": "INPUT", "other": {"anies": [{"name": "referenceToUnitGroupDataSet", "value": {"shortDescription": [{"value": "MJ", "lang": "de"}], "type": "unit group data set", "refObjectId": "93a60a57-a3c8-11da-a746-0800200c9a66", "uri": "../unitgroups/93a60a57-a3c8-11da-a746-0800200c9a66.xml"}}, {"value": "0", "module": "A1-A3"}, {"value": "0", "module": "A4"}, {"value": "0", "module": "A5"}, {"value": "0", "module": "B1"}, {"value": "0", "module": "C1"}, {"value": "0", "module": "C2"}, {"value": "0", "module": "C3"}, {"value": "0", "module": "C4"}, {"value": "0", "module": "D"}]}, "resolvedFlowVersion": "38.00.000", "flowProperties": [], "typeOfFlow": "Other flow", "classification": {"classHierarchy": "Quantities / Environmental quantities / EPD EN 15804 / LCI indicators", "name": "GaBiCategories"}}, {"dataSetInternalID": 10, "referenceToFlowDataSet": {"shortDescription": [{"value": "Einsatz von Süßwasserressourcen (FW)", "lang": "de"}, {"value": "Use of net fresh water (FW)", "lang": "en"}], "type": "flow data set", "refObjectId": "3cf952c8-f3a4-461d-8c96-96456ca62246", "uri": "../flows/3cf952c8-f3a4-461d-8c96-96456ca62246.xml"}, "exchange direction": "INPUT", "other": {"anies": [{"name": "referenceToUnitGroupDataSet", "value": {"shortDescription": [{"value": "m^3", "lang": "de"}], "type": "unit group data set", "refObjectId": "cd950537-0a98-4044-9ba7-9f9a68d0a504", "uri": "../unitgroups/cd950537-0a98-4044-9ba7-9f9a68d0a504.xml"}}, {"value": "0.0008568", "module": "A1-A3"}, {"value": "7.66E-06", "module": "A4"}, {"value": "0.000401", "module": "A5"}, {"value": "0", "module": "B1"}, {"value": "1.94E-07", "module": "C1"}, {"value": "3.97E-06", "module": "C2"}, {"value": "0", "module": "C3"}, {"value": "5.25E-05", "module": "C4"}, {"value": "-3.12E-05", "module": "D"}]}, "resolvedFlowVersion": "38.00.000", "flowProperties": [], "typeOfFlow": "Other flow", "classification": {"classHierarchy": "Quantities / Environmental quantities / EPD EN 15804 / LCI indicators", "name": "GaBiCategories"}}, {"dataSetInternalID": 11, "referenceToFlowDataSet": {"shortDescription": [{"value": "Gefährlicher Abfall zur Deponie (HWD)", "lang": "de"}, {"value": "Hazardous waste disposed (HWD)", "lang": "en"}], "type": "flow data set", "refObjectId": "430f9e0f-59b2-46a0-8e0d-55e0e84948fc", "uri": "../flows/430f9e0f-59b2-46a0-8e0d-55e0e84948fc.xml"}, "exchange direction": "OUTPUT", "other": {"anies": [{"name": "referenceToUnitGroupDataSet", "value": {"shortDescription": [{"value": "kg", "lang": "de"}], "type": "unit group data set", "refObjectId": "ad38d542-3fe9-439d-9b95-2f5f7752acaf", "uri": "../unitgroups/ad38d542-3fe9-439d-9b95-2f5f7752acaf.xml"}}, {"value": "7.64E-10", "module": "A1-A3"}, {"value": "6.84E-13", "module": "A4"}, {"value": "1.15E-12", "module": "A5"}, {"value": "0", "module": "B1"}, {"value": "1.66E-14", "module": "C1"}, {"value": "3.54E-13", "module": "C2"}, {"value": "0", "module": "C3"}, {"value": "1.07E-11", "module": "C4"}, {"value": "-4.11E-11", "module": "D"}]}, "resolvedFlowVersion": "38.00.000", "flowProperties": [], "typeOfFlow": "Other flow", "classification": {"classHierarchy": "Quantities / Environmental quantities / EPD EN 15804 / LCI indicators", "name": "GaBiCategories"}}, {"dataSetInternalID": 12, "referenceToFlowDataSet": {"shortDescription": [{"value": "Entsorgter nicht gefährlicher Abfall (NHWD)", "lang": "de"}, {"value": "Non hazardous waste disposed (NHWD)", "lang": "en"}], "type": "flow data set", "refObjectId": "b29ef66b-e286-4afa-949f-62f1a7b4d7fa", "uri": "../flows/b29ef66b-e286-4afa-949f-62f1a7b4d7fa.xml"}, "exchange direction": "OUTPUT", "other": {"anies": [{"name": "referenceToUnitGroupDataSet", "value": {"shortDescription": [{"value": "kg", "lang": "de"}], "type": "unit group data set", "refObjectId": "ad38d542-3fe9-439d-9b95-2f5f7752acaf", "uri": "../unitgroups/ad38d542-3fe9-439d-9b95-2f5f7752acaf.xml"}}, {"value": "0.00732", "module": "A1-A3"}, {"value": "2.34E-05", "module": "A4"}, {"value": "0.000411", "module": "A5"}, {"value": "0", "module": "B1"}, {"value": "6.19E-07", "module": "C1"}, {"value": "1.21E-05", "module": "C2"}, {"value": "0", "module": "C3"}, {"value": "1.06", "module": "C4"}, {"value": "-0.000139", "module": "D"}]}, "resolvedFlowVersion": "38.00.000", "flowProperties": [], "typeOfFlow": "Other flow", "classification": {"classHierarchy": "Quantities / Environmental quantities / EPD EN 15804 / LCI indicators", "name": "GaBiCategories"}}, {"dataSetInternalID": 13, "referenceToFlowDataSet": {"shortDescription": [{"value": "Entsorgter radioaktiver Abfall (RWD)", "lang": "de"}, {"value": "Radioactive waste disposed (RWD)", "lang": "en"}], "type": "flow data set", "refObjectId": "3449546e-52ad-4b39-b809-9fb77cea8ff6", "uri": "../flows/3449546e-52ad-4b39-b809-9fb77cea8ff6.xml"}, "exchange direction": "OUTPUT", "other": {"anies": [{"name": "referenceToUnitGroupDataSet", "value": {"shortDescription": [{"value": "kg", "lang": "de"}], "type": "unit group data set", "refObjectId": "ad38d542-3fe9-439d-9b95-2f5f7752acaf", "uri": "../unitgroups/ad38d542-3fe9-439d-9b95-2f5f7752acaf.xml"}}, {"value": "6.95E-05", "module": "A1-A3"}, {"value": "1.49E-07", "module": "A4"}, {"value": "4.22E-07", "module": "A5"}, {"value": "0", "module": "B1"}, {"value": "4.78E-09", "module": "C1"}, {"value": "7.71E-08", "module": "C2"}, {"value": "0", "module": "C3"}, {"value": "2.27E-06", "module": "C4"}, {"value": "-8.27E-06", "module": "D"}]}, "resolvedFlowVersion": "38.00.000", "flowProperties": [], "typeOfFlow": "Other flow", "classification": {"classHierarchy": "Quantities / Environmental quantities / EPD EN 15804 / LCI indicators", "name": "GaBiCategories"}}, {"dataSetInternalID": 14, "referenceToFlowDataSet": {"shortDescription": [{"value": "Komponenten für die Wiederverwendung (CRU)", "lang": "de"}, {"value": "Components for re-use (CRU)", "lang": "en"}], "type": "flow data set", "refObjectId": "a2b32f97-3fc7-4af2-b209-525bc6426f33", "uri": "../flows/a2b32f97-3fc7-4af2-b209-525bc6426f33.xml"}, "exchange direction": "OUTPUT", "other": {"anies": [{"name": "referenceToUnitGroupDataSet", "value": {"shortDescription": [{"value": "kg", "lang": "de"}], "type": "unit group data set", "refObjectId": "ad38d542-3fe9-439d-9b95-2f5f7752acaf", "uri": "../unitgroups/ad38d542-3fe9-439d-9b95-2f5f7752acaf.xml"}}, {"value": "0", "module": "A1-A3"}, {"value": "0", "module": "A4"}, {"value": "0", "module": "A5"}, {"value": "0", "module": "B1"}, {"value": "0", "module": "C1"}, {"value": "0", "module": "C2"}, {"value": "0", "module": "C3"}, {"value": "0", "module": "C4"}, {"value": "0", "module": "D"}]}, "resolvedFlowVersion": "38.00.000", "flowProperties": [], "typeOfFlow": "Other flow", "classification": {"classHierarchy": "Quantities / Environmental quantities / EPD EN 15804 / LCI indicators", "name": "GaBiCategories"}}, {"dataSetInternalID": 15, "referenceToFlowDataSet": {"shortDescription": [{"value": "Stoffe zum Recycling (MFR)", "lang": "de"}, {"value": "Materials for recycling (MFR)", "lang": "en"}], "type": "flow data set", "refObjectId": "d7fe48a5-4103-49c8-9aae-b0b5dfdbd6ae", "uri": "../flows/d7fe48a5-4103-49c8-9aae-b0b5dfdbd6ae.xml"}, "exchange direction": "OUTPUT", "other": {"anies": [{"name": "referenceToUnitGroupDataSet", "value": {"shortDescription": [{"value": "kg", "lang": "de"}], "type": "unit group data set", "refObjectId": "ad38d542-3fe9-439d-9b95-2f5f7752acaf", "uri": "../unitgroups/ad38d542-3fe9-439d-9b95-2f5f7752acaf.xml"}}, {"value": "0", "module": "A1-A3"}, {"value": "0", "module": "A4"}, {"value": "0", "module": "A5"}, {"value": "0", "module": "B1"}, {"value": "0", "module": "C1"}, {"value": "0", "module": "C2"}, {"value": "0", "module": "C3"}, {"value": "0", "module": "C4"}, {"value": "0", "module": "D"}]}, "resolvedFlowVersion": "38.00.000", "flowProperties": [], "typeOfFlow": "Other flow", "classification": {"classHierarchy": "Quantities / Environmental quantities / EPD EN 15804 / LCI indicators", "name": "GaBiCategories"}}, {"dataSetInternalID": 16, "referenceToFlowDataSet": {"shortDescription": [{"value": "Stoffe für die Energierückgewinnung (MER)", "lang": "de"}, {"value": "Materials for energy recovery (MER)", "lang": "en"}], "type": "flow data set", "refObjectId": "59a9181c-3aaf-46ee-8b13-2b3723b6e447", "uri": "../flows/59a9181c-3aaf-46ee-8b13-2b3723b6e447.xml"}, "exchange direction": "OUTPUT", "other": {"anies": [{"name": "referenceToUnitGroupDataSet", "value": {"shortDescription": [{"value": "kg", "lang": "de"}], "type": "unit group data set", "refObjectId": "ad38d542-3fe9-439d-9b95-2f5f7752acaf", "uri": "../unitgroups/ad38d542-3fe9-439d-9b95-2f5f7752acaf.xml"}}, {"value": "0", "module": "A1-A3"}, {"value": "0", "module": "A4"}, {"value": "0", "module": "A5"}, {"value": "0", "module": "B1"}, {"value": "0", "module": "C1"}, {"value": "0", "module": "C2"}, {"value": "0", "module": "C3"}, {"value": "0", "module": "C4"}, {"value": "0", "module": "D"}]}, "resolvedFlowVersion": "38.00.000", "flowProperties": [], "typeOfFlow": "Other flow", "classification": {"classHierarchy": "Quantities / Environmental quantities / EPD EN 15804 / LCI indicators", "name": "GaBiCategories"}}, {"dataSetInternalID": 17, "referenceToFlowDataSet": {"shortDescription": [{"value": "Exportierte elektrische Energie (EEE)", "lang": "de"}, {"value": "Exported electrical energy (EEE)", "lang": "en"}], "type": "flow data set", "refObjectId": "4da0c987-2b76-40d6-9e9e-82a017aaaf29", "uri": "../flows/4da0c987-2b76-40d6-9e9e-82a017aaaf29.xml"}, "exchange direction": "OUTPUT", "other": {"anies": [{"name": "referenceToUnitGroupDataSet", "value": {"shortDescription": [{"value": "MJ", "lang": "de"}], "type": "unit group data set", "refObjectId": "93a60a57-a3c8-11da-a746-0800200c9a66", "uri": "../unitgroups/93a60a57-a3c8-11da-a746-0800200c9a66.xml"}}, {"value": "0", "module": "A1-A3"}, {"value": "0", "module": "A4"}, {"value": "0.0522", "module": "A5"}, {"value": "0", "module": "B1"}, {"value": "0", "module": "C1"}, {"value": "0", "module": "C2"}, {"value": "0", "module": "C3"}, {"value": "0", "module": "C4"}, {"value": "0", "module": "D"}]}, "resolvedFlowVersion": "38.00.000", "flowProperties": [], "typeOfFlow": "Other flow", "classification": {"classHierarchy": "Quantities / Environmental quantities / EPD EN 15804 / LCI indicators", "name": "GaBiCategories"}}, {"dataSetInternalID": 18, "referenceToFlowDataSet": {"shortDescription": [{"value": "Exportierte thermische Energie (EET)", "lang": "de"}, {"value": "Exported thermal energy (EET)", "lang": "en"}], "type": "flow data set", "refObjectId": "98daf38a-7a79-46d3-9a37-2b7bd0955810", "uri": "../flows/98daf38a-7a79-46d3-9a37-2b7bd0955810.xml"}, "exchange direction": "OUTPUT", "other": {"anies": [{"name": "referenceToUnitGroupDataSet", "value": {"shortDescription": [{"value": "MJ", "lang": "de"}], "type": "unit group data set", "refObjectId": "93a60a57-a3c8-11da-a746-0800200c9a66", "uri": "../unitgroups/93a60a57-a3c8-11da-a746-0800200c9a66.xml"}}, {"value": "0", "module": "A1-A3"}, {"value": "0", "module": "A4"}, {"value": "0.122", "module": "A5"}, {"value": "0", "module": "B1"}, {"value": "0", "module": "C1"}, {"value": "0", "module": "C2"}, {"value": "0", "module": "C3"}, {"value": "0", "module": "C4"}, {"value": "0", "module": "D"}]}, "resolvedFlowVersion": "38.00.000", "flowProperties": [], "typeOfFlow": "Other flow", "classification": {"classHierarchy": "Quantities / Environmental quantities / EPD EN 15804 / LCI indicators", "name": "GaBiCategories"}}]}, "LCIAResults": {"LCIAResult": [{"referenceToLCIAMethodDataSet": {"shortDescription": [{"value": "Globales Erwärmungspotenzial total (GWP-total)", "lang": "de"}, {"value": "Global Warming Potential total (GWP-total)", "lang": "en"}], "type": "LCIA method data set", "refObjectId": "6a37f984-a4b3-458a-a20a-64418c145fa2", "uri": "../lciamethods/6a37f984-a4b3-458a-a20a-64418c145fa2.xml"}, "other": {"anies": [{"name": "referenceToUnitGroupDataSet", "value": {"shortDescription": [{"value": "kg CO_(2)-Äq.", "lang": "de"}], "type": "unit group data set", "refObjectId": "1ebf3012-d0db-4de2-aefd-ef30cedb0be1", "uri": "../unitgroups/1ebf3012-d0db-4de2-aefd-ef30cedb0be1.xml"}}, {"value": "0.335", "module": "A1-A3"}, {"value": "0.0112", "module": "A4"}, {"value": "0.0416", "module": "A5"}, {"value": "-0.162", "module": "B1"}, {"value": "0.000284", "module": "C1"}, {"value": "0.00579", "module": "C2"}, {"value": "0", "module": "C3"}, {"value": "0.0154", "module": "C4"}, {"value": "-0.0163", "module": "D"}]}}, {"referenceToLCIAMethodDataSet": {"shortDescription": [{"value": "Globales Erwärmungspotenzial fossil (GWP-fossil)", "lang": "de"}, {"value": "Global Warming Potential fossil fuels (GWP-fossil)", "lang": "en"}], "type": "LCIA method data set", "refObjectId": "5f635281-343e-44fb-83df-1971b155e6b6", "uri": "../lciamethods/5f635281-343e-44fb-83df-1971b155e6b6.xml"}, "other": {"anies": [{"name": "referenceToUnitGroupDataSet", "value": {"shortDescription": [{"value": "kg CO_(2)-Äq.", "lang": "de"}], "type": "unit group data set", "refObjectId": "1ebf3012-d0db-4de2-aefd-ef30cedb0be1", "uri": "../unitgroups/1ebf3012-d0db-4de2-aefd-ef30cedb0be1.xml"}}, {"value": "0.368", "module": "A1-A3"}, {"value": "0.0111", "module": "A4"}, {"value": "0.0035", "module": "A5"}, {"value": "-0.162", "module": "B1"}, {"value": "0.000284", "module": "C1"}, {"value": "0.00576", "module": "C2"}, {"value": "0", "module": "C3"}, {"value": "0.0158", "module": "C4"}, {"value": "-0.0161", "module": "D"}]}}, {"referenceToLCIAMethodDataSet": {"shortDescription": [{"value": "Globales Erwärmungspotenzial biogen (GWP-biogenic)", "lang": "de"}, {"value": "Global Warming Potential biogenic (GWP-biogenic)", "lang": "en"}], "type": "LCIA method data set", "refObjectId": "2356e1ab-0185-4db5-86e5-16de51c7485c", "uri": "../lciamethods/2356e1ab-0185-4db5-86e5-16de51c7485c.xml"}, "other": {"anies": [{"name": "referenceToUnitGroupDataSet", "value": {"shortDescription": [{"value": "kg CO_(2)-Äq.", "lang": "de"}], "type": "unit group data set", "refObjectId": "1ebf3012-d0db-4de2-aefd-ef30cedb0be1", "uri": "../unitgroups/1ebf3012-d0db-4de2-aefd-ef30cedb0be1.xml"}}, {"value": "-0.0325", "module": "A1-A3"}, {"value": "4.58E-06", "module": "A4"}, {"value": "0.0381", "module": "A5"}, {"value": "0", "module": "B1"}, {"value": "-1.2E-06", "module": "C1"}, {"value": "2.37E-06", "module": "C2"}, {"value": "0", "module": "C3"}, {"value": "-0.000468", "module": "C4"}, {"value": "-0.000115", "module": "D"}]}}, {"referenceToLCIAMethodDataSet": {"shortDescription": [{"value": "Globales Erwärmungspotenzial luluc (GWP-luluc)", "lang": "de"}, {"value": "Global Warming Potential luluc (GWP-luluc)", "lang": "en"}], "type": "LCIA method data set", "refObjectId": "4331bbdb-978a-490d-8707-eeb047f01a55", "uri": "../lciamethods/4331bbdb-978a-490d-8707-eeb047f01a55.xml"}, "other": {"anies": [{"name": "referenceToUnitGroupDataSet", "value": {"shortDescription": [{"value": "kg CO_(2)-Äq.", "lang": "de"}], "type": "unit group data set", "refObjectId": "1ebf3012-d0db-4de2-aefd-ef30cedb0be1", "uri": "../unitgroups/1ebf3012-d0db-4de2-aefd-ef30cedb0be1.xml"}}, {"value": "0.000126", "module": "A1-A3"}, {"value": "4.15E-05", "module": "A4"}, {"value": "1.52E-07", "module": "A5"}, {"value": "0", "module": "B1"}, {"value": "1.1E-06", "module": "C1"}, {"value": "2.15E-05", "module": "C2"}, {"value": "0", "module": "C3"}, {"value": "2.92E-05", "module": "C4"}, {"value": "-2.8E-06", "module": "D"}]}}, {"referenceToLCIAMethodDataSet": {"shortDescription": [{"value": "Abbau Potential der stratosphärischen Ozonschicht (ODP)", "lang": "de"}, {"value": "Depletion potential of the stratospheric ozone layer (ODP)", "lang": "en"}], "type": "LCIA method data set", "refObjectId": "b5c629d6-def3-11e6-bf01-fe55135034f3", "uri": "../lciamethods/b5c629d6-def3-11e6-bf01-fe55135034f3.xml"}, "other": {"anies": [{"name": "referenceToUnitGroupDataSet", "value": {"shortDescription": [{"value": "kg CFC11-Äq.", "lang": "de"}], "type": "unit group data set", "refObjectId": "d9e957c9-7309-4474-bf3a-7777df6c4e5b", "uri": "../unitgroups/d9e957c9-7309-4474-bf3a-7777df6c4e5b.xml"}}, {"value": "1.14E-12", "module": "A1-A3"}, {"value": "1.59E-15", "module": "A4"}, {"value": "6.21E-15", "module": "A5"}, {"value": "0", "module": "B1"}, {"value": "5.88E-17", "module": "C1"}, {"value": "8.22E-16", "module": "C2"}, {"value": "0", "module": "C3"}, {"value": "3.76E-14", "module": "C4"}, {"value": "-1.6E-13", "module": "D"}]}}, {"referenceToLCIAMethodDataSet": {"shortDescription": [{"value": "Versauerungspotenzial von Boden und Wasser (AP)", "lang": "de"}, {"value": "Acidification potential of land and water (AP)", "lang": "en"}], "type": "LCIA method data set", "refObjectId": "b5c611c6-def3-11e6-bf01-fe55135034f3", "uri": "../lciamethods/b5c611c6-def3-11e6-bf01-fe55135034f3.xml"}, "other": {"anies": [{"name": "referenceToUnitGroupDataSet", "value": {"shortDescription": [{"value": "mol H^(+)-Äq.", "lang": "de"}], "type": "unit group data set", "refObjectId": "42e089ac-92bf-4bf2-8ca1-5fc40d18f2ed", "uri": "../unitgroups/42e089ac-92bf-4bf2-8ca1-5fc40d18f2ed.xml"}}, {"value": "0.000387", "module": "A1-A3"}, {"value": "1.07E-05", "module": "A4"}, {"value": "8.04E-06", "module": "A5"}, {"value": "0", "module": "B1"}, {"value": "3.83E-06", "module": "C1"}, {"value": "5.52E-06", "module": "C2"}, {"value": "0", "module": "C3"}, {"value": "0.000112", "module": "C4"}, {"value": "-1.65E-05", "module": "D"}]}}, {"referenceToLCIAMethodDataSet": {"shortDescription": [{"value": "Eutrophierungspotenzial Süßwasser (EP-freshwater)", "lang": "de"}, {"value": "Eutrophication potential aquatic freshwater (EP-freshwater)", "lang": "en"}], "type": "LCIA method data set", "refObjectId": "b53ec18f-7377-4ad3-86eb-cc3f4f276b2b", "uri": "../lciamethods/b53ec18f-7377-4ad3-86eb-cc3f4f276b2b.xml"}, "other": {"anies": [{"name": "referenceToUnitGroupDataSet", "value": {"shortDescription": [{"value": "kg P-Äq.", "lang": "de"}], "type": "unit group data set", "refObjectId": "0429039d-a61d-4590-ba67-aa4a20a810a1", "uri": "../unitgroups/0429039d-a61d-4590-ba67-aa4a20a810a1.xml"}}, {"value": "1.41E-06", "module": "A1-A3"}, {"value": "2.3E-08", "module": "A4"}, {"value": "4.84E-09", "module": "A5"}, {"value": "0", "module": "B1"}, {"value": "5.72E-10", "module": "C1"}, {"value": "1.19E-08", "module": "C2"}, {"value": "0", "module": "C3"}, {"value": "2.69E-08", "module": "C4"}, {"value": "-3.31E-08", "module": "D"}]}}, {"referenceToLCIAMethodDataSet": {"shortDescription": [{"value": "Eutrophierungspotenzial Salzwasser (EP-marine)", "lang": "de"}, {"value": "Eutrophication potential aquatic marine (EP-marine)", "lang": "en"}], "type": "LCIA method data set", "refObjectId": "b5c619fa-def3-11e6-bf01-fe55135034f3", "uri": "../lciamethods/b5c619fa-def3-11e6-bf01-fe55135034f3.xml"}, "other": {"anies": [{"name": "referenceToUnitGroupDataSet", "value": {"shortDescription": [{"value": "kg N-Äq.", "lang": "de"}], "type": "unit group data set", "refObjectId": "d05bb823-ecdf-4686-8c40-bf1d9257859f", "uri": "../unitgroups/d05bb823-ecdf-4686-8c40-bf1d9257859f.xml"}}, {"value": "0.000123", "module": "A1-A3"}, {"value": "3.59E-06", "module": "A4"}, {"value": "2.27E-06", "module": "A5"}, {"value": "0", "module": "B1"}, {"value": "1.74E-06", "module": "C1"}, {"value": "1.86E-06", "module": "C2"}, {"value": "0", "module": "C3"}, {"value": "2.87E-05", "module": "C4"}, {"value": "-5.89E-06", "module": "D"}]}}, {"referenceToLCIAMethodDataSet": {"shortDescription": [{"value": "Eutrophierungspotenzial Land (EP-terrestrial)", "lang": "de"}, {"value": "Eutrophication potential terrestrial (EP-terrestrial)", "lang": "en"}], "type": "LCIA method data set", "refObjectId": "b5c614d2-def3-11e6-bf01-fe55135034f3", "uri": "../lciamethods/b5c614d2-def3-11e6-bf01-fe55135034f3.xml"}, "other": {"anies": [{"name": "referenceToUnitGroupDataSet", "value": {"shortDescription": [{"value": "mol N-Äq.", "lang": "de"}], "type": "unit group data set", "refObjectId": "71b4d617-0ec9-4d3f-b65e-e438940c2401", "uri": "../unitgroups/71b4d617-0ec9-4d3f-b65e-e438940c2401.xml"}}, {"value": "0.00137", "module": "A1-A3"}, {"value": "4.29E-05", "module": "A4"}, {"value": "3.8E-05", "module": "A5"}, {"value": "0", "module": "B1"}, {"value": "1.92E-05", "module": "C1"}, {"value": "2.22E-05", "module": "C2"}, {"value": "0", "module": "C3"}, {"value": "0.000315", "module": "C4"}, {"value": "-6.29E-05", "module": "D"}]}}, {"referenceToLCIAMethodDataSet": {"shortDescription": [{"value": "Bildungspotential für troposphärisches Ozon (POCP)", "lang": "de"}, {"value": "Formation potential of tropospheric ozone photochemical oxidants (POCP)", "lang": "en"}], "type": "LCIA method data set", "refObjectId": "b5c610fe-def3-11e6-bf01-fe55135034f3", "uri": "../lciamethods/b5c610fe-def3-11e6-bf01-fe55135034f3.xml"}, "other": {"anies": [{"name": "referenceToUnitGroupDataSet", "value": {"shortDescription": [{"value": "kg NMVOC-Äq.", "lang": "de"}], "type": "unit group data set", "refObjectId": "d27c25f8-fbc1-44c6-b47b-4adbae4199c6", "uri": "../unitgroups/d27c25f8-fbc1-44c6-b47b-4adbae4199c6.xml"}}, {"value": "0.000321", "module": "A1-A3"}, {"value": "9.35E-06", "module": "A4"}, {"value": "5.92E-06", "module": "A5"}, {"value": "0", "module": "B1"}, {"value": "5.22E-06", "module": "C1"}, {"value": "4.84E-06", "module": "C2"}, {"value": "0", "module": "C3"}, {"value": "8.72E-05", "module": "C4"}, {"value": "-1.55E-05", "module": "D"}]}}, {"referenceToLCIAMethodDataSet": {"shortDescription": [{"value": "Potenzial für den abiotischen Abbau nicht fossiler Ressourcen (ADPE)", "lang": "de"}, {"value": "Abiotic depletion potential for non fossil resources (ADPE)", "lang": "en"}], "type": "LCIA method data set", "refObjectId": "b2ad6494-c78d-11e6-9d9d-cec0c932ce01", "uri": "../lciamethods/b2ad6494-c78d-11e6-9d9d-cec0c932ce01.xml"}, "other": {"anies": [{"name": "referenceToUnitGroupDataSet", "value": {"shortDescription": [{"value": "kg Sb-Äq.", "lang": "de"}], "type": "unit group data set", "refObjectId": "54ccd2d9-a32a-4fc2-923d-f2c8c93e89d4", "uri": "../unitgroups/54ccd2d9-a32a-4fc2-923d-f2c8c93e89d4.xml"}}, {"value": "3.94E-07", "module": "A1-A3"}, {"value": "1.15E-09", "module": "A4"}, {"value": "1.52E-10", "module": "A5"}, {"value": "0", "module": "B1"}, {"value": "2.87E-11", "module": "C1"}, {"value": "5.95E-10", "module": "C2"}, {"value": "0", "module": "C3"}, {"value": "1.63E-09", "module": "C4"}, {"value": "-9.43E-09", "module": "D"}]}}, {"referenceToLCIAMethodDataSet": {"shortDescription": [{"value": "Potenzial für den abiotischen Abbau fossiler Brennstoffe (ADPF)", "lang": "de"}, {"value": "Abiotic depletion potential for fossil resources (ADPF)", "lang": "en"}], "type": "LCIA method data set", "refObjectId": "b2ad6110-c78d-11e6-9d9d-cec0c932ce01", "uri": "../lciamethods/b2ad6110-c78d-11e6-9d9d-cec0c932ce01.xml"}, "other": {"anies": [{"name": "referenceToUnitGroupDataSet", "value": {"shortDescription": [{"value": "MJ", "lang": "de"}], "type": "unit group data set", "refObjectId": "93a60a57-a3c8-11da-a746-0800200c9a66", "uri": "../unitgroups/93a60a57-a3c8-11da-a746-0800200c9a66.xml"}}, {"value": "3.25", "module": "A1-A3"}, {"value": "0.148", "module": "A4"}, {"value": "0.0113", "module": "A5"}, {"value": "0", "module": "B1"}, {"value": "0.0038", "module": "C1"}, {"value": "0.0766", "module": "C2"}, {"value": "0", "module": "C3"}, {"value": "0.207", "module": "C4"}, {"value": "-0.232", "module": "D"}]}}, {"referenceToLCIAMethodDataSet": {"shortDescription": [{"value": "Wassernutzung (WDP)", "lang": "de"}, {"value": "Water use (WDP)", "lang": "en"}], "type": "LCIA method data set", "refObjectId": "b2ad66ce-c78d-11e6-9d9d-cec0c932ce01", "uri": "../lciamethods/b2ad66ce-c78d-11e6-9d9d-cec0c932ce01.xml"}, "other": {"anies": [{"name": "referenceToUnitGroupDataSet", "value": {"shortDescription": [{"value": "m^(3) Welt-Äq. entzogen", "lang": "de"}], "type": "unit group data set", "refObjectId": "6ae2df01-888e-46c8-b17d-49fa3869b476", "uri": "../unitgroups/6ae2df01-888e-46c8-b17d-49fa3869b476.xml"}}, {"value": "0.00851", "module": "A1-A3"}, {"value": "4.38E-05", "module": "A4"}, {"value": "0.00469", "module": "A5"}, {"value": "0", "module": "B1"}, {"value": "1.23E-06", "module": "C1"}, {"value": "2.27E-05", "module": "C2"}, {"value": "0", "module": "C3"}, {"value": "0.00173", "module": "C4"}, {"value": "-0.000197", "module": "D"}]}}, {"referenceToLCIAMethodDataSet": {"shortDescription": [{"value": "Auftreten von Krankheiten aufgrund von Feinstaubemissionen (PM)", "lang": "de"}, {"value": "Incidence of disease due to PM emissions (PM)", "lang": "en"}], "type": "LCIA method data set", "refObjectId": "b5c602c6-def3-11e6-bf01-fe55135034f3", "uri": "../lciamethods/b5c602c6-def3-11e6-bf01-fe55135034f3.xml"}, "other": {"anies": [{"name": "referenceToUnitGroupDataSet", "value": {"shortDescription": [{"value": "Krankheitsfälle", "lang": "de"}], "type": "unit group data set", "refObjectId": "3883559b-648f-4afc-8ba2-0bd24f3affa3", "uri": "../unitgroups/3883559b-648f-4afc-8ba2-0bd24f3affa3.xml"}}, {"value": "1.57E-08", "module": "A1-A3"}, {"value": "6.3E-11", "module": "A4"}, {"value": "4.43E-11", "module": "A5"}, {"value": "0", "module": "B1"}, {"value": "2.05E-10", "module": "C1"}, {"value": "3.26E-11", "module": "C2"}, {"value": "0", "module": "C3"}, {"value": "1.38E-09", "module": "C4"}, {"value": "-1.28E-10", "module": "D"}]}}, {"referenceToLCIAMethodDataSet": {"shortDescription": [{"value": "Wirkung durch Exposition des Menschen mit U235 (IR)", "lang": "de"}, {"value": "Human exposure efficiency relative to U235 (IR)", "lang": "en"}], "type": "LCIA method data set", "refObjectId": "b5c632be-def3-11e6-bf01-fe55135034f3", "uri": "../lciamethods/b5c632be-def3-11e6-bf01-fe55135034f3.xml"}, "other": {"anies": [{"name": "referenceToUnitGroupDataSet", "value": {"shortDescription": [{"value": "kBq U235-Äq.", "lang": "de"}], "type": "unit group data set", "refObjectId": "456b05bf-1415-44a9-9993-02452f554c09", "uri": "../unitgroups/456b05bf-1415-44a9-9993-02452f554c09.xml"}}, {"value": "0.00685", "module": "A1-A3"}, {"value": "1.45E-05", "module": "A4"}, {"value": "3.94E-05", "module": "A5"}, {"value": "0", "module": "B1"}, {"value": "4.86E-07", "module": "C1"}, {"value": "7.5E-06", "module": "C2"}, {"value": "0", "module": "C3"}, {"value": "0.000247", "module": "C4"}, {"value": "-0.00082", "module": "D"}]}}, {"referenceToLCIAMethodDataSet": {"shortDescription": [{"value": "Toxizitätsvergleichseinheit für Ökosysteme (ETP-fw)", "lang": "de"}, {"value": "Comparative toxic unit for ecosystems (ETP-fw)", "lang": "en"}], "type": "LCIA method data set", "refObjectId": "ee1082d1-b0f7-43ca-a1f0-21e2a4a74511", "uri": "../lciamethods/ee1082d1-b0f7-43ca-a1f0-21e2a4a74511.xml"}, "other": {"anies": [{"name": "referenceToUnitGroupDataSet", "value": {"shortDescription": [{"value": "CTUe", "lang": "de"}], "type": "unit group data set", "refObjectId": "aa959ded-f1eb-4efb-9c5c-2d60be36b3e6", "uri": "../unitgroups/aa959ded-f1eb-4efb-9c5c-2d60be36b3e6.xml"}}, {"value": "1.37", "module": "A1-A3"}, {"value": "0.117", "module": "A4"}, {"value": "0.00562", "module": "A5"}, {"value": "0", "module": "B1"}, {"value": "0.00292", "module": "C1"}, {"value": "0.0607", "module": "C2"}, {"value": "0", "module": "C3"}, {"value": "0.116", "module": "C4"}, {"value": "-0.0383", "module": "D"}]}}, {"referenceToLCIAMethodDataSet": {"shortDescription": [{"value": "Toxizitätsvergleichseinheit für Menschen (krebserregend) (HTP-c)", "lang": "de"}, {"value": "Comparative toxic unit for humans (carcinogenic) (HTP-c)", "lang": "en"}], "type": "LCIA method data set", "refObjectId": "2299222a-bbd8-474f-9d4f-4dd1f18aea7c", "uri": "../lciamethods/2299222a-bbd8-474f-9d4f-4dd1f18aea7c.xml"}, "other": {"anies": [{"name": "referenceToUnitGroupDataSet", "value": {"shortDescription": [{"value": "CTUh", "lang": "de"}], "type": "unit group data set", "refObjectId": "d4c9523e-2d7e-49fd-8469-998f547d3a70", "uri": "../unitgroups/d4c9523e-2d7e-49fd-8469-998f547d3a70.xml"}}, {"value": "6.73E-11", "module": "A1-A3"}, {"value": "2.33E-12", "module": "A4"}, {"value": "3.08E-13", "module": "A5"}, {"value": "0", "module": "B1"}, {"value": "5.84E-14", "module": "C1"}, {"value": "1.21E-12", "module": "C2"}, {"value": "0", "module": "C3"}, {"value": "1.77E-11", "module": "C4"}, {"value": "-3.06E-12", "module": "D"}]}}, {"referenceToLCIAMethodDataSet": {"shortDescription": [{"value": "Toxizitätsvergleichseinheit für Menschen (nicht krebserregend) (HTP-nc)", "lang": "de"}, {"value": "Comparative toxic unit for humans (noncarcinogenic) (HTP-nc)", "lang": "en"}], "type": "LCIA method data set", "refObjectId": "3af763a5-b7a1-48c9-9cee-1f223481fcef", "uri": "../lciamethods/3af763a5-b7a1-48c9-9cee-1f223481fcef.xml"}, "other": {"anies": [{"name": "referenceToUnitGroupDataSet", "value": {"shortDescription": [{"value": "CTUh", "lang": "de"}], "type": "unit group data set", "refObjectId": "d4c9523e-2d7e-49fd-8469-998f547d3a70", "uri": "../unitgroups/d4c9523e-2d7e-49fd-8469-998f547d3a70.xml"}}, {"value": "6.23E-09", "module": "A1-A3"}, {"value": "1.16E-10", "module": "A4"}, {"value": "1.32E-11", "module": "A5"}, {"value": "0", "module": "B1"}, {"value": "4.39E-12", "module": "C1"}, {"value": "6.02E-11", "module": "C2"}, {"value": "0", "module": "C3"}, {"value": "1.96E-09", "module": "C4"}, {"value": "-1.17E-10", "module": "D"}]}}, {"referenceToLCIAMethodDataSet": {"shortDescription": [{"value": "Bodenqualitätsindex (SQP)", "lang": "de"}, {"value": "Soil quality index (SQP)", "lang": "en"}], "type": "LCIA method data set", "refObjectId": "b2ad6890-c78d-11e6-9d9d-cec0c932ce01", "uri": "../lciamethods/b2ad6890-c78d-11e6-9d9d-cec0c932ce01.xml"}, "other": {"anies": [{"name": "referenceToUnitGroupDataSet", "value": {"shortDescription": [{"value": "SQP", "lang": "de"}], "type": "unit group data set", "refObjectId": "f130951c-e67f-4f7f-8dd4-665de3974e18", "uri": "../unitgroups/f130951c-e67f-4f7f-8dd4-665de3974e18.xml"}}, {"value": "6.64", "module": "A1-A3"}, {"value": "0.0464", "module": "A4"}, {"value": "0.00308", "module": "A5"}, {"value": "0", "module": "B1"}, {"value": "0.00114", "module": "C1"}, {"value": "0.0241", "module": "C2"}, {"value": "0", "module": "C3"}, {"value": "0.0451", "module": "C4"}, {"value": "-0.0507", "module": "D"}]}}]}, "otherAttributes": {"{http://www.indata.network/EPD/2019}epd-version": "1.2"}, "version": "1.1", "locations": "../ILCDLocations.xml"}