{"processInformation": {"dataSetInformation": {"UUID": "0347f3ef-4113-4ae9-987f-6f3b324f35c7", "name": {"baseName": [{"value": "Hilti CFS-F FX", "lang": "en"}, {"value": "Hilti CFS-F FX", "lang": "de"}], "functionalUnitFlowProperties": [{"lang": "en"}]}, "classificationInformation": {"classification": [{"class": [{"value": "Dämmstoffe", "level": 0, "classId": "2"}, {"value": "Polyethylen", "level": 1, "classId": "2.18"}, {"value": "Schaum", "level": 2, "classId": "2.18.01"}], "name": "OEKOBAU.DAT"}, {"class": [{"value": "02 Building products", "level": 0}, {"value": "Construction adhesives and coatings", "level": 1}, {"value": "Reaction resin products", "level": 2}], "name": "IBUCategories"}]}, "generalComment": [{"lang": "en"}]}, "quantitativeReference": {"referenceToReferenceFlow": [0]}, "time": {"referenceYear": 2022, "dataSetValidUntil": 2027, "other": {"anies": [{"name": "publicationDateOfEPD", "value": 1663718400000}]}}, "geography": {"locationOfOperationSupplyOrProduction": {"location": "GLO"}}, "technology": {"technologyDescriptionAndIncludedProcesses": [{"value": "Most raw materials are sourced in Europe. The transport is exclusively by truck for the European raw materials, and by truck and by ship for the others. The production of the chemical firestop foam consists of a mixing process and a filling process of the respective single components (A and B) and their subsequent combination in a two-component system (packaging). Here process control technology is used to weigh and mix solid and liquid compounds according to the specification. In the next step both well-mixed components run through an automized filling line in which each of the processed masses is filled into a tubular foil bag. Finally the single components are combined in one packaging unit. The two-pack foil bags are packed into cardboard boxes and then finally shipped. The manufacturing plant of CFS-F FX, Hilti GmbH Industriegesellschaft für Befestigungstechnik, Hiltistr. 6, 86916 Kaufering, Germany, is certified according to ISO 9001. The guideline defines international standards for quality and process management. The following flowcharts illustrate the underlying production process Illustration: Production process of the reaction resin mixture Illustration: Production process of the packaging \nDeclared unit: \nThe declared product is a HILTI firestop foam CFS-F FX. The declared unit refers to one kilogram of reaction resin product in the required mixing ratio of the two components. The packaging of 0,267 kg/kg of product is also included in the calculation. 1 package of CFS-F FX contains 0.41kg of reaction resin. The following table shows the data of the declared unit.", "lang": "en"}, {"value": "Die meisten Rohstoffe werden in Europa beschafft. Der Transport erfolgt bei den europäischen Rohstoffen ausschließlich per LKW, bei den anderen per LKW und per Schiff.\n\nDie Herstellung des chemischen Brandschutzschaums besteht aus einem Misch- und Abfüllprozess der jeweiligen Einzelkomponenten (A und B) und deren anschließender Zusammenführung zu einem Zweikomponentensystem (Verpackung). Dabei werden die festen und flüssigen Komponenten mit Hilfe von Prozessleittechnik entsprechend der Spezifikation abgewogen und gemischt. Im nächsten Schritt durchlaufen die beiden gut gemischten Komponenten eine automatisierte Abfüllanlage, in der jede der verarbeiteten Massen in einen Folienschlauchbeutel abgefüllt wird. Abschließend werden die einzelnen Komponenten in einer Verpackungseinheit zusammengeführt. Die Folienbeutel im Zweierpack werden in Kartons verpackt und schließlich versandt. Die Produktionsstätte des CFS-F FX, die Hilti GmbH Industriegesellschaft für Befestigungstechnik, Hiltistr. 6, 86916 Kaufering, Deutschland, ist nach ISO 9001 zertifiziert. Die Richtlinie definiert internationale Standards für Qualitäts- und Prozessmanagement.  \n\nDie folgenden Flussdiagramme veranschaulichen den zugrunde liegenden Produktionsprozess\n\n\nAbbildung: Herstellungsprozess der Reaktionsharzmischung\n\n\nAbbildung: Herstellungsprozess der Verpackung \n", "lang": "de"}], "technologicalApplicability": [{"value": "Hilti CFS-F FX serves to form a penetration seal, which is used to maintain the fire resistance of a concrete, masonry or drywall separating element (wall or floor) when and where services (cables, metal or plastic pipes, etc.) pass through.", "lang": "en"}, {"value": "Hilti CFS-F FX dient als Abschottung zur Aufrechterhaltung des Feuerwiderstandes eines Trennelements aus Beton, Mauerwerk oder Trockenbau (Wand oder Boden), wenn und wo Leitungen (Kabel, Metall- oder Kunststoffrohre usw.) hindurchgeführt werden.  ", "lang": "de"}]}}, "modellingAndValidation": {"LCIMethodAndAllocation": {"typeOfDataSet": "EPD", "referenceToLCAMethodDetails": [{"shortDescription": [{"value": "Reaction resin products.pdf", "lang": "en"}], "type": "source data set", "refObjectId": "c47e21f8-3b6d-42a8-9509-0f577850c591"}], "other": {"anies": [{"name": "subType", "value": "average dataset"}]}}, "dataSourcesTreatmentAndRepresentativeness": {"referenceToDataSource": [{"shortDescription": [{"value": "ecoinvent database (all versions)", "lang": "en"}], "type": "source data set", "refObjectId": "b497a91f-e14b-4b69-8f28-f50eb1576766"}, {"shortDescription": [{"value": "ecoinvent 3.8 database", "lang": "en"}], "type": "source data set", "refObjectId": "0f4c65c0-6210-450f-b886-82bf8dd5ace9"}], "useAdviceForDataSet": [{"value": "Scope: \nThis document refers to the CFS-F-FX firestop foam  with its packaging. Specific data from 2021 were collected from Hilti's manufacturing plant in Kaufering, Germany and used for this environmental Life Cycle Assessment.\n\n\nThe owner of the declaration shall be liable for the underlying information and evidence; the IBU shall not be liable with respect to manufacturer information, life cycle assessment data and evidences. The EPD was created according to the specifications of EN 15804+A2. In the following, the standard will be simplified as EN 15804. \nSystem boundary: \nThe type of EPD is cradle to grave. The following information modules are defined as system boundaries in this study: \n\n\nA1 – Raw material supply:  \n\nProduction and packaging of the raw materials to be supplied to the manufacturer. All processes are included from cradle to gate. \n\nA2 – Transport (to manufacturing site):  \n\nTransportation of all the raw materials and their packaging between their production site and the manufacturing site, for all transport modes (sea, road).  \n\nA3 – Manufacturing:  \n\nProduction, supply and use of energy sources at the manufacturing sites (electricity, biomass and natural gas). Green electricity  from wind turbines is considered for the whole manufacturing process. \n\nProduction and transport of production losses, final product packaging and other inputs.  \n\nEnd-of-life of production waste (hazardous, non-hazardous and recyclable), production losses and raw material packaging,  including waste and losses transportation, processing and disposal. \n\nA4 – Transport (to construction site) \n\nTransportation of packaged products from the manufacturing site to the construction site, including potential in-betweens (retailer, workshop, etc.). \n\nA5 – Installation-Construction \n\nElectricity consumption for injecting (in case of injection with electrical dispenser). \n\nProduction of the construction losses. \n\nProvision and end-of-life of tools and accessories for injectable mortars (manual or electrical dispenser with or without battery and with cartridge holder). \n\nEnd-of-life of hazardous construction losses and packaging (uncured resin and soiled packaging) and non-hazardous construction losses (cured foam and unsoiled packaging): including waste transportation, processing and disposal. \n\nC1 – Deconstruction/demolition \n\nDiesel for building demolition.  \n\nC2 – Transport (to waste processing) \n\nTransportation to waste processing facility. \n\nC4– Waste disposal  \n\nTreatment and disposal of plastic to sanitary landfill. \n\n\nFor the environmental impact, the use of green electricity (stage A3) was calculated taking into account the residual electricity mix for the remaining electricity. The proportion of the electricity demand covered by green electricity in the total electricity demand is 100%.", "lang": "en"}], "other": {"anies": [{"name": "referenceToOriginalEPD", "value": {"shortDescription": {"value": "Hilti CFS-F FX.pdf", "defaultValue": "Hilti CFS-F FX.pdf", "lstrings": [{"lang": "en", "value": "Hilti CFS-F FX.pdf"}]}, "type": "source data set", "uuid": {"uuid": "22f73a3a-0a15-4ad7-ae81-ad921f85608c"}, "refObjectId": "22f73a3a-0a15-4ad7-ae81-ad921f85608c", "resourceURLs": ["https://oekobaudat.de/OEKOBAU.DAT/resource/sources/22f73a3a-0a15-4ad7-ae81-ad921f85608c/Hilti_CFS-F_FX_16050.pdf?version=00.01.000"]}}]}}, "validation": {"review": [{"referenceToNameOfReviewerAndInstitution": [{"shortDescription": [{"value": "Institut Bauen und Umwelt e. V.", "lang": "en"}], "type": "contact data set", "refObjectId": "d111dbec-b024-4be5-86c5-752d6eb2cf95", "uri": "../contacts/d111dbec-b024-4be5-86c5-752d6eb2cf95.xml"}], "type": "Accredited third party review"}]}, "complianceDeclarations": {"compliance": [{"referenceToComplianceSystem": {"shortDescription": [{"value": "DIN EN 15804+A2", "lang": "en"}], "type": "source data set", "refObjectId": "c0016b33-8cf7-415c-ac6e-deba0d21440d", "uri": "../sources/c0016b33-8cf7-415c-ac6e-deba0d21440d.xml"}}, {"referenceToComplianceSystem": {"shortDescription": [{"value": "ISO 14025", "lang": "en"}], "type": "source data set", "refObjectId": "4f2eb655-6e44-4874-a95a-e28f5442cd4d", "uri": "../sources/4f2eb655-6e44-4874-a95a-e28f5442cd4d.xml"}}]}}, "administrativeInformation": {"commissionerAndGoal": {"referenceToCommissioner": [{"shortDescription": [{"value": "Hilti Aktiengesellschaft", "lang": "en"}], "type": "contact data set", "refObjectId": "71be6bd4-8792-49c8-bedb-37bd69a50203", "uri": "../contacts/71be6bd4-8792-49c8-bedb-37bd69a50203.xml"}]}, "dataGenerator": {"referenceToPersonOrEntityGeneratingTheDataSet": [{"shortDescription": [{"value": "Hilti Aktiengesellschaft", "lang": "en"}], "type": "contact data set", "refObjectId": "71be6bd4-8792-49c8-bedb-37bd69a50203", "uri": "../contacts/71be6bd4-8792-49c8-bedb-37bd69a50203.xml"}]}, "dataEntryBy": {"timeStamp": 1663769200705, "referenceToDataSetFormat": [{"shortDescription": [{"value": "ILCD Format", "lang": "en"}], "type": "source data set", "refObjectId": "a97a0155-0234-4b87-b4ce-a45da52f2a40", "uri": "../sources/a97a0155-0234-4b87-b4ce-a45da52f2a40.xml"}, {"shortDescription": [{"value": "EPD-Datenformaterweiterungen v1.2", "lang": "de"}, {"value": "EPD Data Format Extensions v1.2", "lang": "en"}], "type": "source data set", "refObjectId": "a29449fd-aa2f-4de8-b5d7-4b06b43c6fde", "uri": "../sources/a29449fd-aa2f-4de8-b5d7-4b06b43c6fde.xml"}]}, "publicationAndOwnership": {"dataSetVersion": "00.01.000", "referenceToRegistrationAuthority": {"shortDescription": [{"value": "Institut Bauen und Umwelt e. V.", "lang": "en"}], "type": "contact data set", "refObjectId": "d111dbec-b024-4be5-86c5-752d6eb2cf95", "uri": "../contacts/d111dbec-b024-4be5-86c5-752d6eb2cf95.xml"}, "registrationNumber": "EPD-HIL-20220211-ICA1-EN", "referenceToOwnershipOfDataSet": {"shortDescription": [{"value": "Hilti Aktiengesellschaft", "lang": "en"}], "type": "contact data set", "refObjectId": "71be6bd4-8792-49c8-bedb-37bd69a50203", "uri": "../contacts/71be6bd4-8792-49c8-bedb-37bd69a50203.xml"}, "copyright": true, "licenseType": "Free of charge for all users and uses", "accessRestrictions": [{"value": "None", "lang": "en"}], "other": {"anies": [{"name": "referenceToPublisher", "value": {"shortDescription": [{"value": "Institut Bauen und Umwelt e. V.", "lang": "en"}], "type": "contact data set", "refObjectId": "d111dbec-b024-4be5-86c5-752d6eb2cf95", "uri": "../contacts/d111dbec-b024-4be5-86c5-752d6eb2cf95.xml"}}]}}}, "exchanges": {"exchange": [{"dataSetInternalID": 0, "referenceToFlowDataSet": {"shortDescription": [{"value": "CFS-F-FX ()", "lang": "en"}], "type": "flow data set", "refObjectId": "eba9c5c0-241f-3d19-226a-cb28861b0999", "uri": "../flows/eba9c5c0-241f-3d19-226a-cb28861b0999.xml"}, "meanAmount": 1.0, "referencesToDataSource": {}, "referenceFlow": true, "resolvedFlowVersion": "00.01.000", "resultingflowAmount": 1.0, "flowProperties": [{"name": [{"lang": "en", "value": "Mass"}, {"lang": "de", "value": "Masse"}], "uuid": "93a60a56-a3c8-11da-a746-0800200b9a66", "referenceFlowProperty": true, "meanValue": 1.0, "referenceUnit": "kg", "unitGroupUUID": "ad38d542-3fe9-439d-9b95-2f5f7752acaf"}], "materialProperties": [{"name": "gross density", "value": "1260.0", "unit": "kg/m^3", "unitDescription": "kilograms per cubic metre"}], "typeOfFlow": "Product flow", "classification": {"classHierarchy": "Dämmstoffe / Polyethylen / Schaum", "name": "OEKOBAU.DAT"}}, {"dataSetInternalID": 1, "referenceToFlowDataSet": {"shortDescription": [{"value": "Renewable primary energy as energy carrier (PERE)", "lang": "en"}, {"value": "Erneuerbare Primärenergie als Energieträger (PERE)", "lang": "de"}], "type": "flow data set", "refObjectId": "20f32be5-0398-4288-9b6d-accddd195317", "uri": "../flows/20f32be5-0398-4288-9b6d-accddd195317.xml"}, "exchange direction": "INPUT", "other": {"anies": [{"name": "referenceToUnitGroupDataSet", "value": {"shortDescription": [{"value": "MJ", "lang": "en"}], "type": "unit group data set", "refObjectId": "93a60a57-a3c8-11da-a746-0800200c9a66", "uri": "../unitgroups/93a60a57-a3c8-11da-a746-0800200c9a66.xml"}}, {"value": "4.14354628038909", "module": "A1"}, {"value": "0.00752757848416981", "module": "A2"}, {"value": "1.07826316068615", "module": "A3"}, {"value": "0.0170213382966125", "module": "A4"}, {"value": "0.344574855279854", "module": "A5"}, {"value": "0.000308913822874431", "module": "C1"}, {"value": "0.00104320478671329", "module": "C2"}, {"value": "0", "module": "C3"}, {"value": "0.0117252398300413", "module": "C4"}, {"value": "0", "module": "D"}]}, "resolvedFlowVersion": "38.00.000", "flowProperties": [], "typeOfFlow": "Other flow", "classification": {"classHierarchy": "Quantities", "name": "GaBiCategories"}}, {"dataSetInternalID": 2, "referenceToFlowDataSet": {"shortDescription": [{"value": "Renewable primary energy resources as material utilization (PERM)", "lang": "en"}, {"value": "Erneuerbare Primärenergie zur stofflichen Nutzung (PERM)", "lang": "de"}], "type": "flow data set", "refObjectId": "fb3ec0de-548d-4508-aea5-00b73bf6f702", "uri": "../flows/fb3ec0de-548d-4508-aea5-00b73bf6f702.xml"}, "exchange direction": "INPUT", "other": {"anies": [{"name": "referenceToUnitGroupDataSet", "value": {"shortDescription": [{"value": "MJ", "lang": "en"}], "type": "unit group data set", "refObjectId": "93a60a57-a3c8-11da-a746-0800200c9a66", "uri": "../unitgroups/93a60a57-a3c8-11da-a746-0800200c9a66.xml"}}, {"value": "0.01324785", "module": "A1"}, {"value": "0", "module": "A2"}, {"value": "0.7327324785", "module": "A3"}, {"value": "0", "module": "A4"}, {"value": "0.02983921314", "module": "A5"}, {"value": "0", "module": "C1"}, {"value": "0", "module": "C2"}, {"value": "0", "module": "C3"}, {"value": "0", "module": "C4"}, {"value": "0", "module": "D"}]}, "resolvedFlowVersion": "38.00.000", "flowProperties": [], "typeOfFlow": "Other flow", "classification": {"classHierarchy": "Quantities", "name": "GaBiCategories"}}, {"dataSetInternalID": 3, "referenceToFlowDataSet": {"shortDescription": [{"value": "Total use of renewable primary energy resources (PERT)", "lang": "en"}, {"value": "Total erneuerbare Primärenergie (PERT)", "lang": "de"}], "type": "flow data set", "refObjectId": "53f97275-fa8a-4cdd-9024-65936002acd0", "uri": "../flows/53f97275-fa8a-4cdd-9024-65936002acd0.xml"}, "exchange direction": "INPUT", "other": {"anies": [{"name": "referenceToUnitGroupDataSet", "value": {"shortDescription": [{"value": "MJ", "lang": "en"}], "type": "unit group data set", "refObjectId": "93a60a57-a3c8-11da-a746-0800200c9a66", "uri": "../unitgroups/93a60a57-a3c8-11da-a746-0800200c9a66.xml"}}, {"value": "4.15679413038909", "module": "A1"}, {"value": "0.00752757848416981", "module": "A2"}, {"value": "1.81099563918615", "module": "A3"}, {"value": "0.0170213382966125", "module": "A4"}, {"value": "0.374414068419854", "module": "A5"}, {"value": "0.000308913822874431", "module": "C1"}, {"value": "0.00104320478671329", "module": "C2"}, {"value": "0", "module": "C3"}, {"value": "0.0117252398300413", "module": "C4"}, {"value": "0", "module": "D"}]}, "resolvedFlowVersion": "38.00.000", "flowProperties": [], "typeOfFlow": "Other flow", "classification": {"classHierarchy": "Quantities / Environmental quantities / EPD EN 15804 / LCI indicators", "name": "GaBiCategories"}}, {"dataSetInternalID": 4, "referenceToFlowDataSet": {"shortDescription": [{"value": "Non renewable primary energy as energy carrier (PENRE)", "lang": "en"}, {"value": "Nicht-erneuerbare Primärenergie als Energieträger (PENRE)", "lang": "de"}], "type": "flow data set", "refObjectId": "ac857178-2b45-46ec-892a-a9a4332f0372", "uri": "../flows/ac857178-2b45-46ec-892a-a9a4332f0372.xml"}, "exchange direction": "INPUT", "other": {"anies": [{"name": "referenceToUnitGroupDataSet", "value": {"shortDescription": [{"value": "MJ", "lang": "en"}], "type": "unit group data set", "refObjectId": "93a60a57-a3c8-11da-a746-0800200c9a66", "uri": "../unitgroups/93a60a57-a3c8-11da-a746-0800200c9a66.xml"}}, {"value": "47.3062265453517", "module": "A1"}, {"value": "0.573827966837651", "module": "A2"}, {"value": "13.89436607014", "module": "A3"}, {"value": "1.17006043760737", "module": "A4"}, {"value": "5.5113078142874", "module": "A5"}, {"value": "0.0540556697322197", "module": "C1"}, {"value": "0.0717107331976816", "module": "C2"}, {"value": "0", "module": "C3"}, {"value": "0.221989077563813", "module": "C4"}, {"value": "0", "module": "D"}]}, "resolvedFlowVersion": "38.00.000", "flowProperties": [], "typeOfFlow": "Other flow", "classification": {"classHierarchy": "Quantities", "name": "GaBiCategories"}}, {"dataSetInternalID": 5, "referenceToFlowDataSet": {"shortDescription": [{"value": "Non renewable primary energy as material utilization (PENRM)", "lang": "en"}, {"value": "Nicht-erneuerbare Primärenergie zur stofflichen Nutzung (PENRM)", "lang": "de"}], "type": "flow data set", "refObjectId": "1421caa0-679d-4bf4-b282-0eb850ccae27", "uri": "../flows/1421caa0-679d-4bf4-b282-0eb850ccae27.xml"}, "exchange direction": "INPUT", "other": {"anies": [{"name": "referenceToUnitGroupDataSet", "value": {"shortDescription": [{"value": "MJ", "lang": "en"}], "type": "unit group data set", "refObjectId": "93a60a57-a3c8-11da-a746-0800200c9a66", "uri": "../unitgroups/93a60a57-a3c8-11da-a746-0800200c9a66.xml"}}, {"value": "24.555875", "module": "A1"}, {"value": "0", "module": "A2"}, {"value": "5.45965293960245", "module": "A3"}, {"value": "0", "module": "A4"}, {"value": "1.24271749469017", "module": "A5"}, {"value": "0", "module": "C1"}, {"value": "0", "module": "C2"}, {"value": "0", "module": "C3"}, {"value": "0", "module": "C4"}, {"value": "0", "module": "D"}]}, "resolvedFlowVersion": "38.00.000", "flowProperties": [], "typeOfFlow": "Other flow", "classification": {"classHierarchy": "Quantities", "name": "GaBiCategories"}}, {"dataSetInternalID": 6, "referenceToFlowDataSet": {"shortDescription": [{"value": "Total use of non renewable primary energy resources (PENRT)", "lang": "en"}, {"value": "Total nicht erneuerbare Primärenergie (PENRT)", "lang": "de"}], "type": "flow data set", "refObjectId": "06159210-646b-4c8d-8583-da9b3b95a6c1", "uri": "../flows/06159210-646b-4c8d-8583-da9b3b95a6c1.xml"}, "exchange direction": "INPUT", "other": {"anies": [{"name": "referenceToUnitGroupDataSet", "value": {"shortDescription": [{"value": "MJ", "lang": "en"}], "type": "unit group data set", "refObjectId": "93a60a57-a3c8-11da-a746-0800200c9a66", "uri": "../unitgroups/93a60a57-a3c8-11da-a746-0800200c9a66.xml"}}, {"value": "71.8621015453517", "module": "A1"}, {"value": "0.573827966837651", "module": "A2"}, {"value": "19.3540190097424", "module": "A3"}, {"value": "1.17006043760737", "module": "A4"}, {"value": "6.75402530897757", "module": "A5"}, {"value": "0.0540556697322197", "module": "C1"}, {"value": "0.0717107331976816", "module": "C2"}, {"value": "0", "module": "C3"}, {"value": "0.221989077563813", "module": "C4"}, {"value": "0", "module": "D"}]}, "resolvedFlowVersion": "38.00.000", "flowProperties": [], "typeOfFlow": "Other flow", "classification": {"classHierarchy": "Quantities / Environmental quantities / EPD EN 15804 / LCI indicators", "name": "GaBiCategories"}}, {"dataSetInternalID": 7, "referenceToFlowDataSet": {"shortDescription": [{"value": "Use of secondary material (SM)", "lang": "en"}, {"value": "Einsatz von Sekundärstoffen (SM)", "lang": "de"}], "type": "flow data set", "refObjectId": "c6a1f35f-2d09-4f54-8dfb-97e502e1ce92", "uri": "../flows/c6a1f35f-2d09-4f54-8dfb-97e502e1ce92.xml"}, "exchange direction": "INPUT", "other": {"anies": [{"name": "referenceToUnitGroupDataSet", "value": {"shortDescription": [{"value": "kg", "lang": "en"}], "type": "unit group data set", "refObjectId": "ad38d542-3fe9-439d-9b95-2f5f7752acaf", "uri": "../unitgroups/ad38d542-3fe9-439d-9b95-2f5f7752acaf.xml"}}, {"value": "0.0252030225290149", "module": "A1"}, {"value": "0.000222198522901741", "module": "A2"}, {"value": "0.090417906282474", "module": "A3"}, {"value": "0.000398277232891563", "module": "A4"}, {"value": "0.0066226420233607", "module": "A5"}, {"value": "2.11542036926058E-05", "module": "C1"}, {"value": "2.44096385696118E-05", "module": "C2"}, {"value": "0", "module": "C3"}, {"value": "8.41290170820906E-05", "module": "C4"}, {"value": "0", "module": "D"}]}, "resolvedFlowVersion": "38.00.000", "flowProperties": [], "typeOfFlow": "Other flow", "classification": {"classHierarchy": "Quantities / Environmental quantities / EPD EN 15804 / LCI indicators", "name": "GaBiCategories"}}, {"dataSetInternalID": 8, "referenceToFlowDataSet": {"shortDescription": [{"value": "Use of renewable secondary fuels (RSF)", "lang": "en"}, {"value": "Erneuerbare Sekundärbrennstoffe (RSF)", "lang": "de"}], "type": "flow data set", "refObjectId": "64333088-a55f-4aa2-9a31-c10b07816787", "uri": "../flows/64333088-a55f-4aa2-9a31-c10b07816787.xml"}, "exchange direction": "INPUT", "other": {"anies": [{"name": "referenceToUnitGroupDataSet", "value": {"shortDescription": [{"value": "MJ", "lang": "en"}], "type": "unit group data set", "refObjectId": "93a60a57-a3c8-11da-a746-0800200c9a66", "uri": "../unitgroups/93a60a57-a3c8-11da-a746-0800200c9a66.xml"}}, {"value": "0.000493119076907894", "module": "A1"}, {"value": "1.85937773233468E-06", "module": "A2"}, {"value": "0.00842229408272263", "module": "A3"}, {"value": "4.38309460972937E-06", "module": "A4"}, {"value": "0.000390319079418584", "module": "A5"}, {"value": "6.91327733208197E-08", "module": "C1"}, {"value": "2.68631361283553E-07", "module": "C2"}, {"value": "0", "module": "C3"}, {"value": "3.83093443829271E-06", "module": "C4"}, {"value": "0", "module": "D"}]}, "resolvedFlowVersion": "38.00.000", "flowProperties": [], "typeOfFlow": "Other flow", "classification": {"classHierarchy": "Quantities / Environmental quantities / EPD EN 15804 / LCI indicators", "name": "GaBiCategories"}}, {"dataSetInternalID": 9, "referenceToFlowDataSet": {"shortDescription": [{"value": "Use of non renewable secondary fuels (NRSF)", "lang": "en"}, {"value": "Nicht erneuerbare Sekundärbrennstoffe (NRSF)", "lang": "de"}], "type": "flow data set", "refObjectId": "89def144-d39a-4287-b86f-efde453ddcb2", "uri": "../flows/89def144-d39a-4287-b86f-efde453ddcb2.xml"}, "exchange direction": "INPUT", "other": {"anies": [{"name": "referenceToUnitGroupDataSet", "value": {"shortDescription": [{"value": "MJ", "lang": "en"}], "type": "unit group data set", "refObjectId": "93a60a57-a3c8-11da-a746-0800200c9a66", "uri": "../unitgroups/93a60a57-a3c8-11da-a746-0800200c9a66.xml"}}, {"value": "0", "module": "A1"}, {"value": "0", "module": "A2"}, {"value": "0", "module": "A3"}, {"value": "0", "module": "A4"}, {"value": "0", "module": "A5"}, {"value": "0", "module": "C1"}, {"value": "0", "module": "C2"}, {"value": "0", "module": "C3"}, {"value": "0", "module": "C4"}, {"value": "0", "module": "D"}]}, "resolvedFlowVersion": "38.00.000", "flowProperties": [], "typeOfFlow": "Other flow", "classification": {"classHierarchy": "Quantities / Environmental quantities / EPD EN 15804 / LCI indicators", "name": "GaBiCategories"}}, {"dataSetInternalID": 10, "referenceToFlowDataSet": {"shortDescription": [{"value": "Use of net fresh water (FW)", "lang": "en"}, {"value": "Einsatz von Süßwasserressourcen (FW)", "lang": "de"}], "type": "flow data set", "refObjectId": "3cf952c8-f3a4-461d-8c96-96456ca62246", "uri": "../flows/3cf952c8-f3a4-461d-8c96-96456ca62246.xml"}, "exchange direction": "INPUT", "other": {"anies": [{"name": "referenceToUnitGroupDataSet", "value": {"shortDescription": [{"value": "m^3", "lang": "en"}], "type": "unit group data set", "refObjectId": "cd950537-0a98-4044-9ba7-9f9a68d0a504", "uri": "../unitgroups/cd950537-0a98-4044-9ba7-9f9a68d0a504.xml"}}, {"value": "0.0713114757112668", "module": "A1"}, {"value": "6.63914458309033E-05", "module": "A2"}, {"value": "0.0100641188332117", "module": "A3"}, {"value": "0.000149165158579256", "module": "A4"}, {"value": "0.00558713267365908", "module": "A5"}, {"value": "3.28244778011065E-06", "module": "C1"}, {"value": "9.1420430479133E-06", "module": "C2"}, {"value": "0", "module": "C3"}, {"value": "0.000291741981689063", "module": "C4"}, {"value": "0", "module": "D"}]}, "resolvedFlowVersion": "38.00.000", "flowProperties": [], "typeOfFlow": "Other flow", "classification": {"classHierarchy": "Quantities / Environmental quantities / EPD EN 15804 / LCI indicators", "name": "GaBiCategories"}}, {"dataSetInternalID": 11, "referenceToFlowDataSet": {"shortDescription": [{"value": "Hazardous waste disposed (HWD)", "lang": "en"}, {"value": "Gefährlicher Abfall zur Deponie (HWD)", "lang": "de"}], "type": "flow data set", "refObjectId": "430f9e0f-59b2-46a0-8e0d-55e0e84948fc", "uri": "../flows/430f9e0f-59b2-46a0-8e0d-55e0e84948fc.xml"}, "exchange direction": "OUTPUT", "other": {"anies": [{"name": "referenceToUnitGroupDataSet", "value": {"shortDescription": [{"value": "kg", "lang": "en"}], "type": "unit group data set", "refObjectId": "ad38d542-3fe9-439d-9b95-2f5f7752acaf", "uri": "../unitgroups/ad38d542-3fe9-439d-9b95-2f5f7752acaf.xml"}}, {"value": "0.559428439688219", "module": "A1"}, {"value": "0.000710493281258126", "module": "A2"}, {"value": "0.0616632916756209", "module": "A3"}, {"value": "0.00133088233524723", "module": "A4"}, {"value": "0.345810429409796", "module": "A5"}, {"value": "7.23264993202179E-05", "module": "C1"}, {"value": "8.15671951575262E-05", "module": "C2"}, {"value": "0", "module": "C3"}, {"value": "0.000346321939029426", "module": "C4"}, {"value": "0", "module": "D"}]}, "resolvedFlowVersion": "38.00.000", "flowProperties": [], "typeOfFlow": "Other flow", "classification": {"classHierarchy": "Quantities / Environmental quantities / EPD EN 15804 / LCI indicators", "name": "GaBiCategories"}}, {"dataSetInternalID": 12, "referenceToFlowDataSet": {"shortDescription": [{"value": "Non hazardous waste disposed (NHWD)", "lang": "en"}, {"value": "Entsorgter nicht gefährlicher Abfall (NHWD)", "lang": "de"}], "type": "flow data set", "refObjectId": "b29ef66b-e286-4afa-949f-62f1a7b4d7fa", "uri": "../flows/b29ef66b-e286-4afa-949f-62f1a7b4d7fa.xml"}, "exchange direction": "OUTPUT", "other": {"anies": [{"name": "referenceToUnitGroupDataSet", "value": {"shortDescription": [{"value": "kg", "lang": "en"}], "type": "unit group data set", "refObjectId": "ad38d542-3fe9-439d-9b95-2f5f7752acaf", "uri": "../unitgroups/ad38d542-3fe9-439d-9b95-2f5f7752acaf.xml"}}, {"value": "6.8446170200659", "module": "A1"}, {"value": "0.01069795366828", "module": "A2"}, {"value": "1.43024263727415", "module": "A3"}, {"value": "0.0236517097361196", "module": "A4"}, {"value": "0.539625392514307", "module": "A5"}, {"value": "0.000508364614718604", "module": "C1"}, {"value": "0.00144956738305258", "module": "C2"}, {"value": "0", "module": "C3"}, {"value": "1.00326999759673", "module": "C4"}, {"value": "0", "module": "D"}]}, "resolvedFlowVersion": "38.00.000", "flowProperties": [], "typeOfFlow": "Other flow", "classification": {"classHierarchy": "Quantities / Environmental quantities / EPD EN 15804 / LCI indicators", "name": "GaBiCategories"}}, {"dataSetInternalID": 13, "referenceToFlowDataSet": {"shortDescription": [{"value": "Radioactive waste disposed (RWD)", "lang": "en"}, {"value": "Entsorgter radioaktiver Abfall (RWD)", "lang": "de"}], "type": "flow data set", "refObjectId": "3449546e-52ad-4b39-b809-9fb77cea8ff6", "uri": "../flows/3449546e-52ad-4b39-b809-9fb77cea8ff6.xml"}, "exchange direction": "OUTPUT", "other": {"anies": [{"name": "referenceToUnitGroupDataSet", "value": {"shortDescription": [{"value": "kg", "lang": "en"}], "type": "unit group data set", "refObjectId": "ad38d542-3fe9-439d-9b95-2f5f7752acaf", "uri": "../unitgroups/ad38d542-3fe9-439d-9b95-2f5f7752acaf.xml"}}, {"value": "0.000153686625650983", "module": "A1"}, {"value": "3.96701000461454E-06", "module": "A2"}, {"value": "3.19574002526856E-05", "module": "A3"}, {"value": "8.05167328550321E-06", "module": "A4"}, {"value": "2.50911882055516E-05", "module": "A5"}, {"value": "3.80503086428119E-07", "module": "C1"}, {"value": "4.93471427811296E-07", "module": "C2"}, {"value": "0", "module": "C3"}, {"value": "1.4732803421208E-06", "module": "C4"}, {"value": "0", "module": "D"}]}, "resolvedFlowVersion": "38.00.000", "flowProperties": [], "typeOfFlow": "Other flow", "classification": {"classHierarchy": "Quantities / Environmental quantities / EPD EN 15804 / LCI indicators", "name": "GaBiCategories"}}, {"dataSetInternalID": 14, "referenceToFlowDataSet": {"shortDescription": [{"value": "Components for re-use (CRU)", "lang": "en"}, {"value": "Komponenten für die Wiederverwendung (CRU)", "lang": "de"}], "type": "flow data set", "refObjectId": "a2b32f97-3fc7-4af2-b209-525bc6426f33", "uri": "../flows/a2b32f97-3fc7-4af2-b209-525bc6426f33.xml"}, "exchange direction": "OUTPUT", "other": {"anies": [{"name": "referenceToUnitGroupDataSet", "value": {"shortDescription": [{"value": "kg", "lang": "en"}], "type": "unit group data set", "refObjectId": "ad38d542-3fe9-439d-9b95-2f5f7752acaf", "uri": "../unitgroups/ad38d542-3fe9-439d-9b95-2f5f7752acaf.xml"}}, {"value": "0", "module": "A1"}, {"value": "0", "module": "A2"}, {"value": "0", "module": "A3"}, {"value": "0", "module": "A4"}, {"value": "0", "module": "A5"}, {"value": "0", "module": "C1"}, {"value": "0", "module": "C2"}, {"value": "0", "module": "C3"}, {"value": "0", "module": "C4"}, {"value": "0", "module": "D"}]}, "resolvedFlowVersion": "38.00.000", "flowProperties": [], "typeOfFlow": "Other flow", "classification": {"classHierarchy": "Quantities / Environmental quantities / EPD EN 15804 / LCI indicators", "name": "GaBiCategories"}}, {"dataSetInternalID": 15, "referenceToFlowDataSet": {"shortDescription": [{"value": "Materials for recycling (MFR)", "lang": "en"}, {"value": "Stoffe zum Recycling (MFR)", "lang": "de"}], "type": "flow data set", "refObjectId": "d7fe48a5-4103-49c8-9aae-b0b5dfdbd6ae", "uri": "../flows/d7fe48a5-4103-49c8-9aae-b0b5dfdbd6ae.xml"}, "exchange direction": "OUTPUT", "other": {"anies": [{"name": "referenceToUnitGroupDataSet", "value": {"shortDescription": [{"value": "kg", "lang": "en"}], "type": "unit group data set", "refObjectId": "ad38d542-3fe9-439d-9b95-2f5f7752acaf", "uri": "../unitgroups/ad38d542-3fe9-439d-9b95-2f5f7752acaf.xml"}}, {"value": "0.000468822821588628", "module": "A1"}, {"value": "1.87779950623847E-05", "module": "A2"}, {"value": "0.0358616279750641", "module": "A3"}, {"value": "3.66699771559929E-06", "module": "A4"}, {"value": "0.095073099215824", "module": "A5"}, {"value": "7.20090936898767E-08", "module": "C1"}, {"value": "2.24743172547202E-07", "module": "C2"}, {"value": "0", "module": "C3"}, {"value": "1.21423300604748E-06", "module": "C4"}, {"value": "0", "module": "D"}]}, "resolvedFlowVersion": "38.00.000", "flowProperties": [], "typeOfFlow": "Other flow", "classification": {"classHierarchy": "Quantities / Environmental quantities / EPD EN 15804 / LCI indicators", "name": "GaBiCategories"}}, {"dataSetInternalID": 16, "referenceToFlowDataSet": {"shortDescription": [{"value": "Materials for energy recovery (MER)", "lang": "en"}, {"value": "Stoffe für die Energierückgewinnung (MER)", "lang": "de"}], "type": "flow data set", "refObjectId": "59a9181c-3aaf-46ee-8b13-2b3723b6e447", "uri": "../flows/59a9181c-3aaf-46ee-8b13-2b3723b6e447.xml"}, "exchange direction": "OUTPUT", "other": {"anies": [{"name": "referenceToUnitGroupDataSet", "value": {"shortDescription": [{"value": "kg", "lang": "en"}], "type": "unit group data set", "refObjectId": "ad38d542-3fe9-439d-9b95-2f5f7752acaf", "uri": "../unitgroups/ad38d542-3fe9-439d-9b95-2f5f7752acaf.xml"}}, {"value": "7.17076641671806E-06", "module": "A1"}, {"value": "1.48342554849612E-08", "module": "A2"}, {"value": "5.92848318251529E-07", "module": "A3"}, {"value": "2.94705116202274E-08", "module": "A4"}, {"value": "4.94384280437757E-07", "module": "A5"}, {"value": "1.15247875008429E-09", "module": "C1"}, {"value": "1.80619045655354E-09", "module": "C2"}, {"value": "0", "module": "C3"}, {"value": "5.84731872933728E-09", "module": "C4"}, {"value": "0", "module": "D"}]}, "resolvedFlowVersion": "38.00.000", "flowProperties": [], "typeOfFlow": "Other flow", "classification": {"classHierarchy": "Quantities / Environmental quantities / EPD EN 15804 / LCI indicators", "name": "GaBiCategories"}}, {"dataSetInternalID": 17, "referenceToFlowDataSet": {"shortDescription": [{"value": "Exported electrical energy (EEE)", "lang": "en"}, {"value": "Exportierte elektrische Energie (EEE)", "lang": "de"}], "type": "flow data set", "refObjectId": "4da0c987-2b76-40d6-9e9e-82a017aaaf29", "uri": "../flows/4da0c987-2b76-40d6-9e9e-82a017aaaf29.xml"}, "exchange direction": "OUTPUT", "other": {"anies": [{"name": "referenceToUnitGroupDataSet", "value": {"shortDescription": [{"value": "MJ", "lang": "en"}], "type": "unit group data set", "refObjectId": "93a60a57-a3c8-11da-a746-0800200c9a66", "uri": "../unitgroups/93a60a57-a3c8-11da-a746-0800200c9a66.xml"}}, {"value": "0.0406811458024085", "module": "A1"}, {"value": "0.000114734430768128", "module": "A2"}, {"value": "0.0108276336101848", "module": "A3"}, {"value": "0.000254765168176491", "module": "A4"}, {"value": "0.00358103308455873", "module": "A5"}, {"value": "2.11954112336406E-05", "module": "C1"}, {"value": "1.56140626722885E-05", "module": "C2"}, {"value": "0", "module": "C3"}, {"value": "0.000453303871682149", "module": "C4"}, {"value": "0", "module": "D"}]}, "resolvedFlowVersion": "38.00.000", "flowProperties": [], "typeOfFlow": "Other flow", "classification": {"classHierarchy": "Quantities / Environmental quantities / EPD EN 15804 / LCI indicators", "name": "GaBiCategories"}}, {"dataSetInternalID": 18, "referenceToFlowDataSet": {"shortDescription": [{"value": "Exported thermal energy (EET)", "lang": "en"}, {"value": "Exportierte thermische Energie (EET)", "lang": "de"}], "type": "flow data set", "refObjectId": "98daf38a-7a79-46d3-9a37-2b7bd0955810", "uri": "../flows/98daf38a-7a79-46d3-9a37-2b7bd0955810.xml"}, "exchange direction": "OUTPUT", "other": {"anies": [{"name": "referenceToUnitGroupDataSet", "value": {"shortDescription": [{"value": "MJ", "lang": "en"}], "type": "unit group data set", "refObjectId": "93a60a57-a3c8-11da-a746-0800200c9a66", "uri": "../unitgroups/93a60a57-a3c8-11da-a746-0800200c9a66.xml"}}, {"value": "0.14186770654297", "module": "A1"}, {"value": "0.000567632680992521", "module": "A2"}, {"value": "0.034031760321549", "module": "A3"}, {"value": "0.00105942859284915", "module": "A4"}, {"value": "0.0121182007363187", "module": "A5"}, {"value": "0.00021455956720392", "module": "C1"}, {"value": "6.49303221628061E-05", "module": "C2"}, {"value": "0", "module": "C3"}, {"value": "0.001222807045117", "module": "C4"}, {"value": "0", "module": "D"}]}, "resolvedFlowVersion": "38.00.000", "flowProperties": [], "typeOfFlow": "Other flow", "classification": {"classHierarchy": "Quantities / Environmental quantities / EPD EN 15804 / LCI indicators", "name": "GaBiCategories"}}]}, "LCIAResults": {"LCIAResult": [{"referenceToLCIAMethodDataSet": {"shortDescription": [{"value": "Global Warming Potential total (GWP-total)", "lang": "en"}, {"value": "Globales Erwärmungspotenzial total (GWP-total)", "lang": "de"}], "type": "LCIA method data set", "refObjectId": "6a37f984-a4b3-458a-a20a-64418c145fa2", "uri": "../lciamethods/6a37f984-a4b3-458a-a20a-64418c145fa2.xml"}, "other": {"anies": [{"name": "referenceToUnitGroupDataSet", "value": {"shortDescription": [{"value": "kg CO_(2)-Äq.", "lang": "en"}], "type": "unit group data set", "refObjectId": "1ebf3012-d0db-4de2-aefd-ef30cedb0be1", "uri": "../unitgroups/1ebf3012-d0db-4de2-aefd-ef30cedb0be1.xml"}}, {"value": "3.34803865507444", "module": "A1"}, {"value": "0.0402577122586627", "module": "A2"}, {"value": "0.886798545079285", "module": "A3"}, {"value": "0.0789171298950515", "module": "A4"}, {"value": "0.755773305620469", "module": "A5"}, {"value": "0.00402168059972286", "module": "C1"}, {"value": "0.00483667771743755", "module": "C2"}, {"value": "0", "module": "C3"}, {"value": "0.114307348827589", "module": "C4"}, {"value": "0", "module": "D"}]}}, {"referenceToLCIAMethodDataSet": {"shortDescription": [{"value": "Global Warming Potential fossil fuels (GWP-fossil)", "lang": "en"}, {"value": "Globales Erwärmungspotenzial fossil (GWP-fossil)", "lang": "de"}], "type": "LCIA method data set", "refObjectId": "5f635281-343e-44fb-83df-1971b155e6b6", "uri": "../lciamethods/5f635281-343e-44fb-83df-1971b155e6b6.xml"}, "other": {"anies": [{"name": "referenceToUnitGroupDataSet", "value": {"shortDescription": [{"value": "kg CO_(2)-Äq.", "lang": "en"}], "type": "unit group data set", "refObjectId": "1ebf3012-d0db-4de2-aefd-ef30cedb0be1", "uri": "../unitgroups/1ebf3012-d0db-4de2-aefd-ef30cedb0be1.xml"}}, {"value": "3.26275084982609", "module": "A1"}, {"value": "0.0401287410934442", "module": "A2"}, {"value": "0.872048171473933", "module": "A3"}, {"value": "0.0786126190171069", "module": "A4"}, {"value": "0.749605525045264", "module": "A5"}, {"value": "0.00401763318869546", "module": "C1"}, {"value": "0.00481801483676728", "module": "C2"}, {"value": "0", "module": "C3"}, {"value": "0.114019717879823", "module": "C4"}, {"value": "0", "module": "D"}]}}, {"referenceToLCIAMethodDataSet": {"shortDescription": [{"value": "Global Warming Potential biogenic (GWP-biogenic)", "lang": "en"}, {"value": "Globales Erwärmungspotenzial biogen (GWP-biogenic)", "lang": "de"}], "type": "LCIA method data set", "refObjectId": "2356e1ab-0185-4db5-86e5-16de51c7485c", "uri": "../lciamethods/2356e1ab-0185-4db5-86e5-16de51c7485c.xml"}, "other": {"anies": [{"name": "referenceToUnitGroupDataSet", "value": {"shortDescription": [{"value": "kg CO_(2)-Äq.", "lang": "en"}], "type": "unit group data set", "refObjectId": "1ebf3012-d0db-4de2-aefd-ef30cedb0be1", "uri": "../unitgroups/1ebf3012-d0db-4de2-aefd-ef30cedb0be1.xml"}}, {"value": "0.0822747383211205", "module": "A1"}, {"value": "0.000107964674021368", "module": "A2"}, {"value": "0.0135060727684887", "module": "A3"}, {"value": "0.000273086644547317", "module": "A4"}, {"value": "0.0058358158211543", "module": "A5"}, {"value": "3.64738200621849E-06", "module": "C1"}, {"value": "1.67369503980735E-05", "module": "C2"}, {"value": "0", "module": "C3"}, {"value": "0.000285483172843197", "module": "C4"}, {"value": "0", "module": "D"}]}}, {"referenceToLCIAMethodDataSet": {"shortDescription": [{"value": "Global Warming Potential luluc (GWP-luluc)", "lang": "en"}, {"value": "Globales Erwärmungspotenzial luluc (GWP-luluc)", "lang": "de"}], "type": "LCIA method data set", "refObjectId": "4331bbdb-978a-490d-8707-eeb047f01a55", "uri": "../lciamethods/4331bbdb-978a-490d-8707-eeb047f01a55.xml"}, "other": {"anies": [{"name": "referenceToUnitGroupDataSet", "value": {"shortDescription": [{"value": "kg CO_(2)-Äq.", "lang": "en"}], "type": "unit group data set", "refObjectId": "1ebf3012-d0db-4de2-aefd-ef30cedb0be1", "uri": "../unitgroups/1ebf3012-d0db-4de2-aefd-ef30cedb0be1.xml"}}, {"value": "0.00301306692723721", "module": "A1"}, {"value": "2.10064911971896E-05", "module": "A2"}, {"value": "0.00124430083686334", "module": "A3"}, {"value": "3.14242333972401E-05", "module": "A4"}, {"value": "0.000331964754050439", "module": "A5"}, {"value": "4.00029021176389E-07", "module": "C1"}, {"value": "1.9259302721996E-06", "module": "C2"}, {"value": "0", "module": "C3"}, {"value": "2.1477749227705E-06", "module": "C4"}, {"value": "0", "module": "D"}]}}, {"referenceToLCIAMethodDataSet": {"shortDescription": [{"value": "Depletion potential of the stratospheric ozone layer (ODP)", "lang": "en"}, {"value": "Abbau Potential der stratosphärischen Ozonschicht (ODP)", "lang": "de"}], "type": "LCIA method data set", "refObjectId": "b5c629d6-def3-11e6-bf01-fe55135034f3", "uri": "../lciamethods/b5c629d6-def3-11e6-bf01-fe55135034f3.xml"}, "other": {"anies": [{"name": "referenceToUnitGroupDataSet", "value": {"shortDescription": [{"value": "kg CFC11-Äq.", "lang": "en"}], "type": "unit group data set", "refObjectId": "d9e957c9-7309-4474-bf3a-7777df6c4e5b", "uri": "../unitgroups/d9e957c9-7309-4474-bf3a-7777df6c4e5b.xml"}}, {"value": "2.62597019008581E-05", "module": "A1"}, {"value": "8.94802351521564E-09", "module": "A2"}, {"value": "3.12589338753946E-07", "module": "A3"}, {"value": "1.82145414925525E-08", "module": "A4"}, {"value": "1.1324242852869E-06", "module": "A5"}, {"value": "8.58748046526841E-10", "module": "C1"}, {"value": "1.11633389465035E-09", "module": "C2"}, {"value": "0", "module": "C3"}, {"value": "3.102127676718E-09", "module": "C4"}, {"value": "0", "module": "D"}]}}, {"referenceToLCIAMethodDataSet": {"shortDescription": [{"value": "Acidification potential of land and water (AP)", "lang": "en"}, {"value": "Versauerungspotenzial von Boden und Wasser (AP)", "lang": "de"}], "type": "LCIA method data set", "refObjectId": "b5c611c6-def3-11e6-bf01-fe55135034f3", "uri": "../lciamethods/b5c611c6-def3-11e6-bf01-fe55135034f3.xml"}, "other": {"anies": [{"name": "referenceToUnitGroupDataSet", "value": {"shortDescription": [{"value": "mol H^(+)-Äq.", "lang": "en"}], "type": "unit group data set", "refObjectId": "42e089ac-92bf-4bf2-8ca1-5fc40d18f2ed", "uri": "../unitgroups/42e089ac-92bf-4bf2-8ca1-5fc40d18f2ed.xml"}}, {"value": "0.0263874173037383", "module": "A1"}, {"value": "0.000373531120310414", "module": "A2"}, {"value": "0.00456984737127654", "module": "A3"}, {"value": "0.000223309776639358", "module": "A4"}, {"value": "0.0026936332376229", "module": "A5"}, {"value": "4.17393002642394E-05", "module": "C1"}, {"value": "1.36862227781711E-05", "module": "C2"}, {"value": "0", "module": "C3"}, {"value": "7.62995469148324E-05", "module": "C4"}, {"value": "0", "module": "D"}]}}, {"referenceToLCIAMethodDataSet": {"shortDescription": [{"value": "Eutrophication potential aquatic freshwater (EP-freshwater)", "lang": "en"}, {"value": "Eutrophierungspotenzial Süßwasser (EP-freshwater)", "lang": "de"}], "type": "LCIA method data set", "refObjectId": "b53ec18f-7377-4ad3-86eb-cc3f4f276b2b", "uri": "../lciamethods/b53ec18f-7377-4ad3-86eb-cc3f4f276b2b.xml"}, "other": {"anies": [{"name": "referenceToUnitGroupDataSet", "value": {"shortDescription": [{"value": "kg PO_(4)-Äq.", "lang": "en"}], "type": "unit group data set", "refObjectId": "0429039d-a61d-4590-ba67-aa4a20a810a1", "uri": "../unitgroups/0429039d-a61d-4590-ba67-aa4a20a810a1.xml"}}, {"value": "0.00155031689307129", "module": "A1"}, {"value": "2.44982380709166E-06", "module": "A2"}, {"value": "0.000279523996344943", "module": "A3"}, {"value": "5.37659487992535E-06", "module": "A4"}, {"value": "0.000242541238267264", "module": "A5"}, {"value": "1.26606419512521E-07", "module": "C1"}, {"value": "3.29521064514213E-07", "module": "C2"}, {"value": "0", "module": "C3"}, {"value": "8.57808383354582E-07", "module": "C4"}, {"value": "0", "module": "D"}]}}, {"referenceToLCIAMethodDataSet": {"shortDescription": [{"value": "Eutrophication potential aquatic marine (EP-marine)", "lang": "en"}, {"value": "Eutrophierungspotenzial Salzwasser (EP-marine)", "lang": "de"}], "type": "LCIA method data set", "refObjectId": "b5c619fa-def3-11e6-bf01-fe55135034f3", "uri": "../lciamethods/b5c619fa-def3-11e6-bf01-fe55135034f3.xml"}, "other": {"anies": [{"name": "referenceToUnitGroupDataSet", "value": {"shortDescription": [{"value": "kg N-Äq.", "lang": "en"}], "type": "unit group data set", "refObjectId": "d05bb823-ecdf-4686-8c40-bf1d9257859f", "uri": "../unitgroups/d05bb823-ecdf-4686-8c40-bf1d9257859f.xml"}}, {"value": "0.00473723098369791", "module": "A1"}, {"value": "8.23891581855561E-05", "module": "A2"}, {"value": "0.000927274299384322", "module": "A3"}, {"value": "4.55812856921308E-05", "module": "A4"}, {"value": "0.000461201531934759", "module": "A5"}, {"value": "1.84998338390185E-05", "module": "C1"}, {"value": "2.79358852928974E-06", "module": "C2"}, {"value": "0", "module": "C3"}, {"value": "0.00213715646120998", "module": "C4"}, {"value": "0", "module": "D"}]}}, {"referenceToLCIAMethodDataSet": {"shortDescription": [{"value": "Eutrophication potential terrestrial (EP-terrestrial)", "lang": "en"}, {"value": "Eutrophierungspotenzial Land (EP-terrestrial)", "lang": "de"}], "type": "LCIA method data set", "refObjectId": "b5c614d2-def3-11e6-bf01-fe55135034f3", "uri": "../lciamethods/b5c614d2-def3-11e6-bf01-fe55135034f3.xml"}, "other": {"anies": [{"name": "referenceToUnitGroupDataSet", "value": {"shortDescription": [{"value": "mol N-Äq.", "lang": "en"}], "type": "unit group data set", "refObjectId": "71b4d617-0ec9-4d3f-b65e-e438940c2401", "uri": "../unitgroups/71b4d617-0ec9-4d3f-b65e-e438940c2401.xml"}}, {"value": "0.0348409873789844", "module": "A1"}, {"value": "0.000912760795412298", "module": "A2"}, {"value": "0.00839078625896411", "module": "A3"}, {"value": "0.000494995563496373", "module": "A4"}, {"value": "0.00583755386966387", "module": "A5"}, {"value": "0.000202619824632486", "module": "C1"}, {"value": "3.0337317327394E-05", "module": "C2"}, {"value": "0", "module": "C3"}, {"value": "0.000306745458873782", "module": "C4"}, {"value": "0", "module": "D"}]}}, {"referenceToLCIAMethodDataSet": {"shortDescription": [{"value": "Formation potential of tropospheric ozone photochemical oxidants (POCP)", "lang": "en"}, {"value": "Bildungspotential für troposphärisches Ozon (POCP)", "lang": "de"}], "type": "LCIA method data set", "refObjectId": "b5c610fe-def3-11e6-bf01-fe55135034f3", "uri": "../lciamethods/b5c610fe-def3-11e6-bf01-fe55135034f3.xml"}, "other": {"anies": [{"name": "referenceToUnitGroupDataSet", "value": {"shortDescription": [{"value": "kg NMVOC-Äq.", "lang": "en"}], "type": "unit group data set", "refObjectId": "d27c25f8-fbc1-44c6-b47b-4adbae4199c6", "uri": "../unitgroups/d27c25f8-fbc1-44c6-b47b-4adbae4199c6.xml"}}, {"value": "0.0129333130789531", "module": "A1"}, {"value": "0.000263505998016719", "module": "A2"}, {"value": "0.00278883404372683", "module": "A3"}, {"value": "0.000190182442992687", "module": "A4"}, {"value": "0.00125323378420479", "module": "A5"}, {"value": "5.57190057263494E-05", "module": "C1"}, {"value": "1.16559127973082E-05", "module": "C2"}, {"value": "0", "module": "C3"}, {"value": "0.0001117727461649", "module": "C4"}, {"value": "0", "module": "D"}]}}, {"referenceToLCIAMethodDataSet": {"shortDescription": [{"value": "Abiotic depletion potential for non fossil resources (ADPE)", "lang": "en"}, {"value": "Potenzial für den abiotischen Abbau nicht fossiler Ressourcen (ADPE)", "lang": "de"}], "type": "LCIA method data set", "refObjectId": "b2ad6494-c78d-11e6-9d9d-cec0c932ce01", "uri": "../lciamethods/b2ad6494-c78d-11e6-9d9d-cec0c932ce01.xml"}, "other": {"anies": [{"name": "referenceToUnitGroupDataSet", "value": {"shortDescription": [{"value": "kg Sb-Äq.", "lang": "en"}], "type": "unit group data set", "refObjectId": "54ccd2d9-a32a-4fc2-923d-f2c8c93e89d4", "uri": "../unitgroups/54ccd2d9-a32a-4fc2-923d-f2c8c93e89d4.xml"}}, {"value": "7.54512588263973E-05", "module": "A1"}, {"value": "1.259549186832E-07", "module": "A2"}, {"value": "4.51007215606473E-06", "module": "A3"}, {"value": "2.84125650919351E-07", "module": "A4"}, {"value": "8.68594736318844E-06", "module": "A5"}, {"value": "2.03521771763841E-09", "module": "C1"}, {"value": "1.74135096725082E-08", "module": "C2"}, {"value": "0", "module": "C3"}, {"value": "3.11122707227237E-08", "module": "C4"}, {"value": "0", "module": "D"}]}}, {"referenceToLCIAMethodDataSet": {"shortDescription": [{"value": "Abiotic depletion potential for fossil resources (ADPF)", "lang": "en"}, {"value": "Potenzial für den abiotischen Abbau fossiler Brennstoffe (ADPF)", "lang": "de"}], "type": "LCIA method data set", "refObjectId": "b2ad6110-c78d-11e6-9d9d-cec0c932ce01", "uri": "../lciamethods/b2ad6110-c78d-11e6-9d9d-cec0c932ce01.xml"}, "other": {"anies": [{"name": "referenceToUnitGroupDataSet", "value": {"shortDescription": [{"value": "MJ", "lang": "en"}], "type": "unit group data set", "refObjectId": "93a60a57-a3c8-11da-a746-0800200c9a66", "uri": "../unitgroups/93a60a57-a3c8-11da-a746-0800200c9a66.xml"}}, {"value": "67.4257995810921", "module": "A1"}, {"value": "0.573796721807004", "module": "A2"}, {"value": "19.3083027875854", "module": "A3"}, {"value": "1.17000850899835", "module": "A4"}, {"value": "6.57453027803198", "module": "A5"}, {"value": "0.0540548656353868", "module": "C1"}, {"value": "0.071707550594025", "module": "C2"}, {"value": "0", "module": "C3"}, {"value": "0.221985178737816", "module": "C4"}, {"value": "0", "module": "D"}]}}, {"referenceToLCIAMethodDataSet": {"shortDescription": [{"value": "Water use (WDP)", "lang": "en"}, {"value": "Wassernutzung (WDP)", "lang": "de"}], "type": "LCIA method data set", "refObjectId": "b2ad66ce-c78d-11e6-9d9d-cec0c932ce01", "uri": "../lciamethods/b2ad66ce-c78d-11e6-9d9d-cec0c932ce01.xml"}, "other": {"anies": [{"name": "referenceToUnitGroupDataSet", "value": {"shortDescription": [{"value": "m^(3) world-Äq. deprived", "lang": "en"}], "type": "unit group data set", "refObjectId": "6ae2df01-888e-46c8-b17d-49fa3869b476", "uri": "../unitgroups/6ae2df01-888e-46c8-b17d-49fa3869b476.xml"}}, {"value": "2.51663835779705", "module": "A1"}, {"value": "0.00252859201633494", "module": "A2"}, {"value": "0.366751813050174", "module": "A3"}, {"value": "0.0054761737577513", "module": "A4"}, {"value": "0.213317714089098", "module": "A5"}, {"value": "0.000145261403238191", "module": "C1"}, {"value": "0.000335624060659013", "module": "C2"}, {"value": "0", "module": "C3"}, {"value": "0.00230065643481459", "module": "C4"}, {"value": "0", "module": "D"}]}}, {"referenceToLCIAMethodDataSet": {"shortDescription": [{"value": "Incidence of disease due to PM emissions (PM)", "lang": "en"}, {"value": "Auftreten von Krankheiten aufgrund von Feinstaubemissionen (PM)", "lang": "de"}], "type": "LCIA method data set", "refObjectId": "b5c602c6-def3-11e6-bf01-fe55135034f3", "uri": "../lciamethods/b5c602c6-def3-11e6-bf01-fe55135034f3.xml"}, "other": {"anies": [{"name": "referenceToUnitGroupDataSet", "value": {"shortDescription": [{"value": "Disease incidence", "lang": "en"}], "type": "unit group data set", "refObjectId": "3883559b-648f-4afc-8ba2-0bd24f3affa3", "uri": "../unitgroups/3883559b-648f-4afc-8ba2-0bd24f3affa3.xml"}}, {"value": "1.95797864582209E-07", "module": "A1"}, {"value": "2.74240204764502E-09", "module": "A2"}, {"value": "4.65662933475232E-08", "module": "A3"}, {"value": "6.3352231598797E-09", "module": "A4"}, {"value": "2.43849870216412E-08", "module": "A5"}, {"value": "1.11873868478358E-09", "module": "C1"}, {"value": "3.88273531147588E-10", "module": "C2"}, {"value": "0", "module": "C3"}, {"value": "1.62228294532332E-09", "module": "C4"}, {"value": "0", "module": "D"}]}}, {"referenceToLCIAMethodDataSet": {"shortDescription": [{"value": "Human exposure efficiency relative to U235 (IR)", "lang": "en"}, {"value": "Wirkung durch Exposition des Menschen mit U235 (IR)", "lang": "de"}], "type": "LCIA method data set", "refObjectId": "b5c632be-def3-11e6-bf01-fe55135034f3", "uri": "../lciamethods/b5c632be-def3-11e6-bf01-fe55135034f3.xml"}, "other": {"anies": [{"name": "referenceToUnitGroupDataSet", "value": {"shortDescription": [{"value": "kBq U235-Äq.", "lang": "en"}], "type": "unit group data set", "refObjectId": "456b05bf-1415-44a9-9993-02452f554c09", "uri": "../unitgroups/456b05bf-1415-44a9-9993-02452f554c09.xml"}}, {"value": "0.418786531807452", "module": "A1"}, {"value": "0.00293227389438774", "module": "A2"}, {"value": "0.0782765058498329", "module": "A3"}, {"value": "0.0061395963360852", "module": "A4"}, {"value": "0.0406407106783061", "module": "A5"}, {"value": "0.000248375137430415", "module": "C1"}, {"value": "0.000376283942818181", "module": "C2"}, {"value": "0", "module": "C3"}, {"value": "0.00147816480193856", "module": "C4"}, {"value": "0", "module": "D"}]}}, {"referenceToLCIAMethodDataSet": {"shortDescription": [{"value": "Comparative toxic unit for ecosystems (ETP-fw)", "lang": "en"}, {"value": "Toxizitätsvergleichseinheit für Ökosysteme (ETP-fw)", "lang": "de"}], "type": "LCIA method data set", "refObjectId": "ee1082d1-b0f7-43ca-a1f0-21e2a4a74511", "uri": "../lciamethods/ee1082d1-b0f7-43ca-a1f0-21e2a4a74511.xml"}, "other": {"anies": [{"name": "referenceToUnitGroupDataSet", "value": {"shortDescription": [{"value": "CTUe", "lang": "en"}], "type": "unit group data set", "refObjectId": "aa959ded-f1eb-4efb-9c5c-2d60be36b3e6", "uri": "../unitgroups/aa959ded-f1eb-4efb-9c5c-2d60be36b3e6.xml"}}, {"value": "235.246455922871", "module": "A1"}, {"value": "0.457429206705126", "module": "A2"}, {"value": "15.5214507019662", "module": "A3"}, {"value": "0.976473155642299", "module": "A4"}, {"value": "23.9562002692842", "module": "A5"}, {"value": "0.0324899190412773", "module": "C1"}, {"value": "0.0598461444283617", "module": "C2"}, {"value": "0", "module": "C3"}, {"value": "0.482533379471391", "module": "C4"}, {"value": "0", "module": "D"}]}}, {"referenceToLCIAMethodDataSet": {"shortDescription": [{"value": "Comparative toxic unit for humans (carcinogenic) (HTP-c)", "lang": "en"}, {"value": "Toxizitätsvergleichseinheit für Menschen (krebserregend) (HTP-c)", "lang": "de"}], "type": "LCIA method data set", "refObjectId": "2299222a-bbd8-474f-9d4f-4dd1f18aea7c", "uri": "../lciamethods/2299222a-bbd8-474f-9d4f-4dd1f18aea7c.xml"}, "other": {"anies": [{"name": "referenceToUnitGroupDataSet", "value": {"shortDescription": [{"value": "CTUh", "lang": "en"}], "type": "unit group data set", "refObjectId": "d4c9523e-2d7e-49fd-8469-998f547d3a70", "uri": "../unitgroups/d4c9523e-2d7e-49fd-8469-998f547d3a70.xml"}}, {"value": "2.87373776853513E-08", "module": "A1"}, {"value": "1.84617903951912E-11", "module": "A2"}, {"value": "6.67457333700292E-10", "module": "A3"}, {"value": "3.00158857518055E-11", "module": "A4"}, {"value": "1.57634200929164E-09", "module": "A5"}, {"value": "1.2452562026263E-12", "module": "C1"}, {"value": "1.83961537853662E-12", "module": "C2"}, {"value": "0", "module": "C3"}, {"value": "7.11842389144528E-12", "module": "C4"}, {"value": "0", "module": "D"}]}}, {"referenceToLCIAMethodDataSet": {"shortDescription": [{"value": "Comparative toxic unit for humans (noncarcinogenic) (HTP-nc)", "lang": "en"}, {"value": "Toxizitätsvergleichseinheit für Menschen (nicht krebserregend) (HTP-nc)", "lang": "de"}], "type": "LCIA method data set", "refObjectId": "3af763a5-b7a1-48c9-9cee-1f223481fcef", "uri": "../lciamethods/3af763a5-b7a1-48c9-9cee-1f223481fcef.xml"}, "other": {"anies": [{"name": "referenceToUnitGroupDataSet", "value": {"shortDescription": [{"value": "CTUh", "lang": "en"}], "type": "unit group data set", "refObjectId": "d4c9523e-2d7e-49fd-8469-998f547d3a70", "uri": "../unitgroups/d4c9523e-2d7e-49fd-8469-998f547d3a70.xml"}}, {"value": "2.84096086621196E-07", "module": "A1"}, {"value": "4.20881908386773E-10", "module": "A2"}, {"value": "1.18152071164591E-08", "module": "A3"}, {"value": "9.55846608837975E-10", "module": "A4"}, {"value": "1.69392063394044E-08", "module": "A5"}, {"value": "2.3490070794889E-11", "module": "C1"}, {"value": "5.85819834097232E-11", "module": "C2"}, {"value": "0", "module": "C3"}, {"value": "1.80610945869833E-10", "module": "C4"}, {"value": "0", "module": "D"}]}}, {"referenceToLCIAMethodDataSet": {"shortDescription": [{"value": "Soil quality index (SQP)", "lang": "en"}, {"value": "Bodenqualitätsindex (SQP)", "lang": "de"}], "type": "LCIA method data set", "refObjectId": "b2ad6890-c78d-11e6-9d9d-cec0c932ce01", "uri": "../lciamethods/b2ad6890-c78d-11e6-9d9d-cec0c932ce01.xml"}, "other": {"anies": [{"name": "referenceToUnitGroupDataSet", "value": {"shortDescription": [{"value": "SQP", "lang": "en"}], "type": "unit group data set", "refObjectId": "f130951c-e67f-4f7f-8dd4-665de3974e18", "uri": "../unitgroups/f130951c-e67f-4f7f-8dd4-665de3974e18.xml"}}, {"value": "12.223568106498", "module": "A1"}, {"value": "0.337013586384724", "module": "A2"}, {"value": "6.87430425157399", "module": "A3"}, {"value": "0.830959816823559", "module": "A4"}, {"value": "1.56725708737884", "module": "A5"}, {"value": "0.00702558821175943", "module": "C1"}, {"value": "0.0509279143255882", "module": "C2"}, {"value": "0", "module": "C3"}, {"value": "0.58299302655433", "module": "C4"}, {"value": "0", "module": "D"}]}}]}, "otherAttributes": {"{http://www.indata.network/EPD/2019}epd-version": "1.2"}, "version": "1.1", "locations": "../ILCDLocations.xml"}