{"processInformation": {"dataSetInformation": {"UUID": "0d8f4d50-c623-4986-b5da-2b95b2d231c8", "name": {"baseName": [{"value": "RS PRO 5100/5150 SC (Steinel GmbH)", "lang": "en"}]}, "classificationInformation": {"classification": [{"class": [{"value": "Gebäudetechnik", "level": 0, "classId": "8"}, {"value": "Elektro", "level": 1, "classId": "8.4"}, {"value": "Beleuchtung", "level": 2, "classId": "8.4.04"}], "name": "OEKOBAU.DAT"}]}, "generalComment": [{"value": "The owner of this EPD shall be liable for the underlying information and evidence. The programme operator Kiwa-Ecobility Experts shall not be liable with respect to manufacturer data, life cycle assessment data and evidence. The environmental product declaration refers to an LED luminaire from the 5100 and 5150 with Sensor. The RS PRO 5150 SC was used as the reference product for this EPD.", "lang": "en"}], "other": {"anies": [{"scenario": [{"description": [{"value": "Generic data from the ecoinvent v.3.6 database (system model allocation, cut-off) were used for primary products, raw materials and supplies as well as energy generation and disposal processes. Purchased parts for which no generic data was available were accounted for on the basis of the material composition, which leads to a neglect of production costs and transportation. The highest proportion of environmental impacts is caused by the use phase, which is, however, based on assumptions about the daily usage time. This assumption is therefore of great importance. For this reason, an average period of use was selected. However, even with a minimum daily usage time, the contribution of the usage phase would dominate. Transport to construction: The customers of Steinel are B2B as well as B2C customers. This means that either partners with their own storage space or customers can be supplied directly. This calculation is very complex. In order to calculate the environmental impact, the example of a building site in Dresden was selected. This meant that the distance to a construction site in Dresden was assumed in the calculation. The distance between our warehouse in Herzebrock-Clarholz and Dresden is 500 km. This calculation and the scenario make it possible to calculate the environmental impact for the distance to your own construction site. Use stage: Unlike described in PCR Part B, the full load hours were determined with the help of an analysis by an external project. Taking the formula into account would make luminaires with sensors look worse in terms of environmental performance. Therefore, in one project,the use phase and full load hours were determined with the help of an analysis by an external project. In this project, the intelligent lighting of the 5100 series was installed in a parking garage. The measurements were used to determine the full load hours of 1009 h/a with sensor. The electricity consumption was balanced for the use phase. Origin of electricity: A European electricity mix was assumed for the usage scenario (market for electricity low voltage - RER)."}], "name": "Standard scenario", "default": true}]}]}}, "quantitativeReference": {"referenceToReferenceFlow": [1], "type": "Reference flow(s)"}, "time": {"referenceYear": 2023, "dataSetValidUntil": 2029, "timeRepresentativenessDescription": [{"value": "The energy consumption data was collected in 2022. The data for the products are current data from 2023.\r", "lang": "en"}], "other": {"anies": [{"name": "publicationDateOfEPD", "value": 1719360000000}]}}, "geography": {"locationOfOperationSupplyOrProduction": {"descriptionOfRestrictions": [{"value": "The results of this EPD are representative for European Union. ", "lang": "en"}], "location": "EU-27"}}, "technology": {"technologyDescriptionAndIncludedProcesses": [{"value": "The RS PRO 5100-Serie is an LED luminaire with a high-frequency sensor. Ideal for parking lots, basements, garages and halls. The RS PRO 5150 SC was used as the reference product for this EPD. For the placing on the market in the European Union/European Free Trade Association (EU/EFTA) (with the exception of Switzerland) the following legal provisions apply:  • Low Voltage Directive 2014/35/EU • Electromagnetic Compatibility Directive 2014/30/EU  • RED Directive 2014/53/EU  • RoHS Directive 2011/65/EU • ERP Directive 2009/125/EC. The CE-marking takes into account the proof of conformity with the respective harmonized standards based on the legal provisions above. For the application and use the respective national provisions apply. The LED luminaires are produced at three locations and then stored in herzebrock clarholz and shipped to customers. The Injection molded parts are produced at the Leipzig-Mölkau site. The resulting production waste, which averages 5%, can normally be reground and reused. However, we consider the 5% to be production waste in our calculation. The Printed circuit boards are produced in Einsiedeln. Here, the PCBs are fitted with electronic components using THT and SMD processes. at the Swiss site in Einsiedeln. The preproducts manufactured in Mölkau and Einsiedeln are assembled and packaged in Curtea de Arges  together with other purchased preproducts and then transported to the dispatch warehouse in Herzebrock-Clarholz. Steinel determined the electricity, gas, oil and water consumption per product for the sites by dividing the annual consumption by the production figures. The activity data collected by the company related to the year 2022. The country-specific electricity mixes (electricity market, low voltage) from the ecoinvent database were used for the locations in Switzerland, Romania and Moldova. The electricity for both German locations is calculated by using the location-based approach.", "lang": "en"}], "technologicalApplicability": [{"value": "parking space / hall / hallway / garage", "lang": "en"}], "referenceToTechnologyFlowDiagrammOrPicture": [{"shortDescription": [{"value": "Flow chart RS PRO 5100/5150 SC (Steinel GmbH)", "lang": "en"}], "type": "source data set", "refObjectId": "057f0003-9398-4998-b1ff-9ded70b16d54", "version": "00.00.001"}]}}, "modellingAndValidation": {"LCIMethodAndAllocation": {"typeOfDataSet": "EPD", "other": {"anies": [{"name": "subType", "value": "specific dataset"}]}}, "dataSourcesTreatmentAndRepresentativeness": {"referenceToDataSource": [{"shortDescription": [{"value": "ecoinvent 3.6 database", "lang": "en"}], "type": "source data set", "refObjectId": "766b9973-5ee8-48a2-8098-72c8e20b369f", "version": "00.00.001"}, {"shortDescription": [{"value": "ecoinvent database (general)", "lang": "en"}], "type": "source data set", "refObjectId": "b497a91f-e14b-4b69-8f28-f50eb1576766", "version": "00.03.002"}], "useAdviceForDataSet": [{"value": "parking space / hall / hallway / garage", "lang": "en"}], "other": {"anies": [{"name": "referenceToOriginalEPD", "value": {"shortDescription": {"value": "RS PRO 5100/5150 SC (Steinel GmbH) EPD", "defaultValue": "RS PRO 5100/5150 SC (Steinel GmbH) EPD", "lstrings": [{"lang": "en", "value": "RS PRO 5100/5150 SC (Steinel GmbH) EPD"}]}, "version": {"version": 1, "majorVersion": 0, "minorVersion": 0, "subMinorVersion": 1, "zero": false, "versionString": "00.00.001"}, "type": "source data set", "uuid": {"uuid": "e2783e8d-331e-4a31-b329-28593c0bb95f"}, "refObjectId": "e2783e8d-331e-4a31-b329-28593c0bb95f", "versionAsString": "00.00.001", "resourceURLs": ["https://oekobaudat.de/OEKOBAU.DAT/resource/sources/e2783e8d-331e-4a31-b329-28593c0bb95f/EPD-Kiwa-EE-175737-EN.pdf?version=00.00.001"]}}]}}, "validation": {"review": [{"reviewDetails": [{"value": "The independent verification is in accordance with the ISO 14025:2011.", "lang": "en"}], "referenceToNameOfReviewerAndInstitution": [{"shortDescription": [{"value": "Elisabet Amat Guasch (External verifier)", "lang": "en"}], "type": "contact data set", "refObjectId": "0b940721-b9a8-4b42-9aae-cba754debb32", "version": "00.00.001"}], "type": "Independent external review"}]}, "complianceDeclarations": {"compliance": [{"referenceToComplianceSystem": {"shortDescription": [{"value": "ISO 14025", "lang": "en"}], "type": "source data set", "refObjectId": "4f2eb655-6e44-4874-a95a-e28f5442cd4d", "version": "00.00.001"}}, {"referenceToComplianceSystem": {"shortDescription": [{"value": "EN 15804+A2", "lang": "de"}, {"value": "EN 15804+A2", "lang": "en"}], "type": "source data set", "refObjectId": "c0016b33-8cf7-415c-ac6e-deba0d21440d", "version": "00.01.000"}}]}}, "administrativeInformation": {"commissionerAndGoal": {"referenceToCommissioner": [{"shortDescription": [{"value": "Steinel GmbH", "lang": "en"}], "type": "contact data set", "refObjectId": "5440e5b7-3a35-4c95-857d-4eb868ea1a68", "version": "00.00.001"}]}, "dataGenerator": {"referenceToPersonOrEntityGeneratingTheDataSet": [{"shortDescription": [{"value": "Steinel GmbH", "lang": "en"}], "type": "contact data set", "refObjectId": "5440e5b7-3a35-4c95-857d-4eb868ea1a68", "version": "00.00.001"}]}, "dataEntryBy": {"timeStamp": 1730797536583, "referenceToDataSetFormat": [{"shortDescription": [{"value": "EPD Data Format Extensions v1.2", "lang": "en"}, {"value": "EPD-Datenformaterweiterungen v1.2", "lang": "de"}], "type": "source data set", "refObjectId": "a29449fd-aa2f-4de8-b5d7-4b06b43c6fde", "version": "00.01.000"}, {"shortDescription": [{"value": "ILCD format", "lang": "en"}], "type": "source data set", "refObjectId": "a97a0155-0234-4b87-b4ce-a45da52f2a40", "version": "01.00.001", "uri": "http://lca.jrc.ec.europa.eu/lcainfohub/sample_data/ilcd/sources/ILCD_Format_a97a0155-0234-4b87-b4ce-a45da52f2a40_01.00.000.xml"}], "referenceToPersonOrEntityEnteringTheData": {"shortDescription": [{"value": "Kiwa GmbH (Berlin)", "lang": "en"}], "type": "contact data set", "refObjectId": "3ea4a87a-3f88-4633-b7e7-1bbdd272be43", "version": "00.00.002"}}, "publicationAndOwnership": {"dataSetVersion": "00.00.004", "referenceToRegistrationAuthority": {"shortDescription": [{"value": "Kiwa-Ecobility Experts, Kiwa GmbH (Berlin)", "lang": "en"}], "type": "contact data set", "refObjectId": "eb52a9a8-9d0f-40ce-a5c9-7b78f5615e5a", "version": "00.00.002"}, "registrationNumber": "EPD-Kiwa-EE-175737-EN", "referenceToOwnershipOfDataSet": {"shortDescription": [{"value": "Steinel GmbH", "lang": "en"}], "type": "contact data set", "refObjectId": "5440e5b7-3a35-4c95-857d-4eb868ea1a68", "version": "00.00.001"}, "copyright": true, "licenseType": "Free of charge for all users and uses", "accessRestrictions": [{"value": "None.", "lang": "en"}], "other": {"anies": [{"name": "referenceToPublisher", "value": {"shortDescription": [{"value": "Kiwa-Ecobility Experts, Kiwa GmbH (Berlin)", "lang": "en"}], "type": "contact data set", "refObjectId": "eb52a9a8-9d0f-40ce-a5c9-7b78f5615e5a", "version": "00.00.002"}}]}}}, "exchanges": {"exchange": [{"dataSetInternalID": 1, "referenceToFlowDataSet": {"shortDescription": [{"value": "RS PRO 5100/5150 SC (Steinel GmbH)", "lang": "en"}], "type": "flow data set", "refObjectId": "7edec00b-c0fb-447a-9926-83ecb026643f", "version": "00.00.001"}, "meanAmount": 1.0, "resultingAmount": 1.0, "referenceFlow": true, "resultingflowAmount": 1.0, "flowProperties": [{"name": [{"lang": "de", "value": "Anzahl"}, {"lang": "en", "value": "Number of pieces"}], "uuid": "01846770-4cfe-4a25-8ad9-919d8d378345", "referenceFlowProperty": true, "meanValue": 1.0, "referenceUnit": "pcs.", "unitGroupUUID": "934110e3-baf4-49e9-992c-3d8109a6aafb"}, {"name": [{"lang": "de", "value": "Masse"}, {"lang": "en", "value": "Mass"}], "uuid": "93a60a56-a3c8-11da-a746-0800200b9a66", "meanValue": 1.726}], "materialProperties": [{"name": "weight per piece", "value": "1.726", "unit": "kg"}], "typeOfFlow": "Product flow", "classification": {"classHierarchy": "Gebäudetechnik / Elektro / Beleuchtung", "name": "OEKOBAU.DAT"}}, {"dataSetInternalID": 2, "referenceToFlowDataSet": {"shortDescription": [{"value": "Komponenten für die Wiederverwendung (CRU)", "lang": "de"}, {"value": "Components for re-use (CRU)", "lang": "en"}, {"value": "Componentes para su reutilización (CRU)", "lang": "es"}, {"value": "Komponenter för återanvändning (CRU)", "lang": "sv"}], "type": "flow data set", "refObjectId": "a2b32f97-3fc7-4af2-b209-525bc6426f33", "version": "30.00.002"}, "exchange direction": "OUTPUT", "meanAmount": 0.0, "other": {"anies": [{"value": "0.0", "module": "A1", "scenario": "Standard scenario"}, {"value": "0.0", "module": "A2", "scenario": "Standard scenario"}, {"value": "0.0", "module": "A3", "scenario": "Standard scenario"}, {"value": "0.0", "module": "A1-A3", "scenario": "Standard scenario"}, {"value": "0.0", "module": "A4", "scenario": "Standard scenario"}, {"value": "0.0", "module": "A5", "scenario": "Standard scenario"}, {"value": "0.0", "module": "B6", "scenario": "Standard scenario"}, {"value": "0.0", "module": "C1", "scenario": "Standard scenario"}, {"value": "0.0", "module": "C2", "scenario": "Standard scenario"}, {"value": "0.0", "module": "C3", "scenario": "Standard scenario"}, {"value": "0.0", "module": "C4", "scenario": "Standard scenario"}, {"value": "0.0", "module": "D", "scenario": "Standard scenario"}, {"name": "referenceToUnitGroupDataSet", "value": {"shortDescription": [{"value": "kg"}], "type": "unit group data set", "refObjectId": "ad38d542-3fe9-439d-9b95-2f5f7752acaf", "uri": "../unitgroups/ad38d542-3fe9-439d-9b95-2f5f7752acaf"}}]}, "resolvedFlowVersion": "38.00.000", "flowProperties": [], "typeOfFlow": "Other flow", "classification": {"classHierarchy": "Quantities / Environmental quantities / EPD EN 15804 / LCI indicators", "name": "GaBiCategories"}}, {"dataSetInternalID": 3, "referenceToFlowDataSet": {"shortDescription": [{"value": "Exportierte elektrische Energie (EEE)", "lang": "de"}, {"value": "Exported electrical energy (EEE)", "lang": "en"}, {"value": "Energía exportada electrica (EEE)", "lang": "es"}, {"value": "Exporterad energi – elektrisk (EEE)", "lang": "sv"}], "type": "flow data set", "refObjectId": "4da0c987-2b76-40d6-9e9e-82a017aaaf29", "version": "30.00.002"}, "exchange direction": "OUTPUT", "meanAmount": 0.0, "other": {"anies": [{"value": "0.0", "module": "A1", "scenario": "Standard scenario"}, {"value": "0.0", "module": "A2", "scenario": "Standard scenario"}, {"value": "-0.0256071063393", "module": "A3", "scenario": "Standard scenario"}, {"value": "-0.0256071063393", "module": "A1-A3", "scenario": "Standard scenario"}, {"value": "0.0", "module": "A4", "scenario": "Standard scenario"}, {"value": "0.0", "module": "A5", "scenario": "Standard scenario"}, {"value": "0.0", "module": "B6", "scenario": "Standard scenario"}, {"value": "0.0", "module": "C1", "scenario": "Standard scenario"}, {"value": "0.0", "module": "C2", "scenario": "Standard scenario"}, {"value": "0.0", "module": "C3", "scenario": "Standard scenario"}, {"value": "0.0", "module": "C4", "scenario": "Standard scenario"}, {"value": "-0.507567866112", "module": "D", "scenario": "Standard scenario"}, {"name": "referenceToUnitGroupDataSet", "value": {"shortDescription": [{"value": "MJ"}], "type": "unit group data set", "refObjectId": "93a60a57-a3c8-11da-a746-0800200c9a66", "uri": "../unitgroups/93a60a57-a3c8-11da-a746-0800200c9a66"}}]}, "resolvedFlowVersion": "38.00.000", "flowProperties": [], "typeOfFlow": "Other flow", "classification": {"classHierarchy": "Quantities / Environmental quantities / EPD EN 15804 / LCI indicators", "name": "GaBiCategories"}}, {"dataSetInternalID": 4, "referenceToFlowDataSet": {"shortDescription": [{"value": "Exportierte thermische Energie (EET)", "lang": "de"}, {"value": "Exported thermal energy (EET)", "lang": "en"}, {"value": "Energía exportada termal (EET)", "lang": "es"}, {"value": "Exporterad energi – termisk (EET)", "lang": "sv"}], "type": "flow data set", "refObjectId": "98daf38a-7a79-46d3-9a37-2b7bd0955810", "version": "30.00.002"}, "exchange direction": "OUTPUT", "meanAmount": 0.0, "other": {"anies": [{"value": "0.0", "module": "A1", "scenario": "Standard scenario"}, {"value": "0.0", "module": "A2", "scenario": "Standard scenario"}, {"value": "-0.04410112758435", "module": "A3", "scenario": "Standard scenario"}, {"value": "-0.04410112758435", "module": "A1-A3", "scenario": "Standard scenario"}, {"value": "0.0", "module": "A4", "scenario": "Standard scenario"}, {"value": "0.0", "module": "A5", "scenario": "Standard scenario"}, {"value": "0.0", "module": "B6", "scenario": "Standard scenario"}, {"value": "0.0", "module": "C1", "scenario": "Standard scenario"}, {"value": "0.0", "module": "C2", "scenario": "Standard scenario"}, {"value": "0.0", "module": "C3", "scenario": "Standard scenario"}, {"value": "0.0", "module": "C4", "scenario": "Standard scenario"}, {"value": "-0.874144658304", "module": "D", "scenario": "Standard scenario"}, {"name": "referenceToUnitGroupDataSet", "value": {"shortDescription": [{"value": "MJ"}], "type": "unit group data set", "refObjectId": "93a60a57-a3c8-11da-a746-0800200c9a66", "uri": "../unitgroups/93a60a57-a3c8-11da-a746-0800200c9a66"}}]}, "resolvedFlowVersion": "38.00.000", "flowProperties": [], "typeOfFlow": "Other flow", "classification": {"classHierarchy": "Quantities / Environmental quantities / EPD EN 15804 / LCI indicators", "name": "GaBiCategories"}}, {"dataSetInternalID": 5, "referenceToFlowDataSet": {"shortDescription": [{"value": "Gefährlicher Abfall zur Deponie (HWD)", "lang": "de"}, {"value": "Hazardous waste disposed (HWD)", "lang": "en"}, {"value": "Residuos peligrosos eliminados (HWD)", "lang": "es"}, {"value": "Farligt avfall (HWD)", "lang": "sv"}], "type": "flow data set", "refObjectId": "430f9e0f-59b2-46a0-8e0d-55e0e84948fc", "version": "30.00.002"}, "exchange direction": "OUTPUT", "meanAmount": 0.0, "other": {"anies": [{"value": "0.0031587058953583", "module": "A1", "scenario": "Standard scenario"}, {"value": "1.47047657835E-5", "module": "A2", "scenario": "Standard scenario"}, {"value": "6.027480915755E-4", "module": "A3", "scenario": "Standard scenario"}, {"value": "0.0037761587527173", "module": "A1-A3", "scenario": "Standard scenario"}, {"value": "5.5355992617E-6", "module": "A4", "scenario": "Standard scenario"}, {"value": "3.318105043E-7", "module": "A5", "scenario": "Standard scenario"}, {"value": "0.0048696285421419", "module": "B6", "scenario": "Standard scenario"}, {"value": "0.0", "module": "C1", "scenario": "Standard scenario"}, {"value": "5.20467925E-7", "module": "C2", "scenario": "Standard scenario"}, {"value": "0.0037756674032855", "module": "C3", "scenario": "Standard scenario"}, {"value": "1.13831706E-8", "module": "C4", "scenario": "Standard scenario"}, {"value": "0.0046287828676316", "module": "D", "scenario": "Standard scenario"}, {"name": "referenceToUnitGroupDataSet", "value": {"shortDescription": [{"value": "kg"}], "type": "unit group data set", "refObjectId": "ad38d542-3fe9-439d-9b95-2f5f7752acaf", "uri": "../unitgroups/ad38d542-3fe9-439d-9b95-2f5f7752acaf"}}]}, "resolvedFlowVersion": "38.00.000", "flowProperties": [], "typeOfFlow": "Other flow", "classification": {"classHierarchy": "Quantities / Environmental quantities / EPD EN 15804 / LCI indicators", "name": "GaBiCategories"}}, {"dataSetInternalID": 6, "referenceToFlowDataSet": {"shortDescription": [{"value": "Stoffe für die Energierückgewinnung (MER)", "lang": "de"}, {"value": "Materials for energy recovery (MER)", "lang": "en"}, {"value": "Materiales para valorización energética (recuperación de energía) (MER)", "lang": "es"}, {"value": "Material till energiåtervinning (MER)", "lang": "sv"}], "type": "flow data set", "refObjectId": "59a9181c-3aaf-46ee-8b13-2b3723b6e447", "version": "30.00.002"}, "exchange direction": "OUTPUT", "meanAmount": 0.0, "other": {"anies": [{"value": "0.0", "module": "A1", "scenario": "Standard scenario"}, {"value": "0.0", "module": "A2", "scenario": "Standard scenario"}, {"value": "0.0", "module": "A3", "scenario": "Standard scenario"}, {"value": "0.0", "module": "A1-A3", "scenario": "Standard scenario"}, {"value": "0.0", "module": "A4", "scenario": "Standard scenario"}, {"value": "0.0", "module": "A5", "scenario": "Standard scenario"}, {"value": "0.0", "module": "B6", "scenario": "Standard scenario"}, {"value": "0.0", "module": "C1", "scenario": "Standard scenario"}, {"value": "0.0", "module": "C2", "scenario": "Standard scenario"}, {"value": "0.0", "module": "C3", "scenario": "Standard scenario"}, {"value": "0.0", "module": "C4", "scenario": "Standard scenario"}, {"value": "0.0", "module": "D", "scenario": "Standard scenario"}, {"name": "referenceToUnitGroupDataSet", "value": {"shortDescription": [{"value": "kg"}], "type": "unit group data set", "refObjectId": "ad38d542-3fe9-439d-9b95-2f5f7752acaf", "uri": "../unitgroups/ad38d542-3fe9-439d-9b95-2f5f7752acaf"}}]}, "resolvedFlowVersion": "38.00.000", "flowProperties": [], "typeOfFlow": "Other flow", "classification": {"classHierarchy": "Quantities / Environmental quantities / EPD EN 15804 / LCI indicators", "name": "GaBiCategories"}}, {"dataSetInternalID": 7, "referenceToFlowDataSet": {"shortDescription": [{"value": "Stoffe zum Recycling (MFR)", "lang": "de"}, {"value": "Materials for recycling (MFR)", "lang": "en"}, {"value": "Materiales para el reciclaje (MFR)", "lang": "es"}, {"value": "Material till återvinning (MFR)", "lang": "sv"}], "type": "flow data set", "refObjectId": "d7fe48a5-4103-49c8-9aae-b0b5dfdbd6ae", "version": "30.00.002"}, "exchange direction": "OUTPUT", "meanAmount": 0.0, "other": {"anies": [{"value": "0.0", "module": "A1", "scenario": "Standard scenario"}, {"value": "0.0", "module": "A2", "scenario": "Standard scenario"}, {"value": "0.0769639555", "module": "A3", "scenario": "Standard scenario"}, {"value": "0.0769639555", "module": "A1-A3", "scenario": "Standard scenario"}, {"value": "0.0", "module": "A4", "scenario": "Standard scenario"}, {"value": "0.0031", "module": "A5", "scenario": "Standard scenario"}, {"value": "0.0", "module": "B6", "scenario": "Standard scenario"}, {"value": "0.0", "module": "C1", "scenario": "Standard scenario"}, {"value": "0.0", "module": "C2", "scenario": "Standard scenario"}, {"value": "1.52686094999999", "module": "C3", "scenario": "Standard scenario"}, {"value": "0.0", "module": "C4", "scenario": "Standard scenario"}, {"value": "0.0", "module": "D", "scenario": "Standard scenario"}, {"name": "referenceToUnitGroupDataSet", "value": {"shortDescription": [{"value": "kg"}], "type": "unit group data set", "refObjectId": "ad38d542-3fe9-439d-9b95-2f5f7752acaf", "uri": "../unitgroups/ad38d542-3fe9-439d-9b95-2f5f7752acaf"}}]}, "resolvedFlowVersion": "38.00.000", "flowProperties": [], "typeOfFlow": "Other flow", "classification": {"classHierarchy": "Quantities / Environmental quantities / EPD EN 15804 / LCI indicators", "name": "GaBiCategories"}}, {"dataSetInternalID": 8, "referenceToFlowDataSet": {"shortDescription": [{"value": "Einsatz von Süßwasserressourcen (FW)", "lang": "de"}, {"value": "Use of net fresh water (FW)", "lang": "en"}, {"value": "Uso neto de recursos de agua dulce (FW)", "lang": "es"}, {"value": "Användning av sötvatten (FW)", "lang": "sv"}], "type": "flow data set", "refObjectId": "3cf952c8-f3a4-461d-8c96-96456ca62246", "version": "30.00.003"}, "exchange direction": "INPUT", "meanAmount": 0.0, "other": {"anies": [{"value": "0.222637335357191", "module": "A1", "scenario": "Standard scenario"}, {"value": "6.695548011027E-4", "module": "A2", "scenario": "Standard scenario"}, {"value": "0.0149770470374538", "module": "A3", "scenario": "Standard scenario"}, {"value": "0.2382839371957475", "module": "A1-A3", "scenario": "Standard scenario"}, {"value": "2.660921464476E-4", "module": "A4", "scenario": "Standard scenario"}, {"value": "3.172027995323E-4", "module": "A5", "scenario": "Standard scenario"}, {"value": "6.11299721658405", "module": "B6", "scenario": "Standard scenario"}, {"value": "0.0", "module": "C1", "scenario": "Standard scenario"}, {"value": "2.50185067196E-5", "module": "C2", "scenario": "Standard scenario"}, {"value": "0.0028907385026945", "module": "C3", "scenario": "Standard scenario"}, {"value": "8.6762193456E-6", "module": "C4", "scenario": "Standard scenario"}, {"value": "-0.0227693864015029", "module": "D", "scenario": "Standard scenario"}, {"name": "referenceToUnitGroupDataSet", "value": {"shortDescription": [{"value": "m3"}], "type": "unit group data set", "refObjectId": "cd950537-0a98-4044-9ba7-9f9a68d0a504", "uri": "../unitgroups/cd950537-0a98-4044-9ba7-9f9a68d0a504"}}]}, "resolvedFlowVersion": "38.00.000", "flowProperties": [], "typeOfFlow": "Other flow", "classification": {"classHierarchy": "Quantities / Environmental quantities / EPD EN 15804 / LCI indicators", "name": "GaBiCategories"}}, {"dataSetInternalID": 9, "referenceToFlowDataSet": {"shortDescription": [{"value": "Entsorgter nicht gefährlicher Abfall (NHWD)", "lang": "de"}, {"value": "Non hazardous waste dispose (NHWD)", "lang": "en"}, {"value": "Residuos no peligrosos eliminados (NHWD)", "lang": "es"}, {"value": "Icke-farligt avfall (NHWD)", "lang": "sv"}], "type": "flow data set", "refObjectId": "b29ef66b-e286-4afa-949f-62f1a7b4d7fa", "version": "30.00.002"}, "exchange direction": "OUTPUT", "meanAmount": 0.0, "other": {"anies": [{"value": "2.20128012578828", "module": "A1", "scenario": "Standard scenario"}, {"value": "0.247910367230934", "module": "A2", "scenario": "Standard scenario"}, {"value": "0.224170901042594", "module": "A3", "scenario": "Standard scenario"}, {"value": "2.673361394061808", "module": "A1-A3", "scenario": "Standard scenario"}, {"value": "0.13856711123703", "module": "A4", "scenario": "Standard scenario"}, {"value": "0.0076040221862587", "module": "A5", "scenario": "Standard scenario"}, {"value": "24.7221471568305", "module": "B6", "scenario": "Standard scenario"}, {"value": "0.0", "module": "C1", "scenario": "Standard scenario"}, {"value": "0.0130283522076192", "module": "C2", "scenario": "Standard scenario"}, {"value": "0.213934487638299", "module": "C3", "scenario": "Standard scenario"}, {"value": "0.0222146734482561", "module": "C4", "scenario": "Standard scenario"}, {"value": "-0.447165498541164", "module": "D", "scenario": "Standard scenario"}, {"name": "referenceToUnitGroupDataSet", "value": {"shortDescription": [{"value": "kg"}], "type": "unit group data set", "refObjectId": "ad38d542-3fe9-439d-9b95-2f5f7752acaf", "uri": "../unitgroups/ad38d542-3fe9-439d-9b95-2f5f7752acaf"}}]}, "resolvedFlowVersion": "38.00.000", "flowProperties": [], "typeOfFlow": "Other flow", "classification": {"classHierarchy": "Quantities / Environmental quantities / EPD EN 15804 / LCI indicators", "name": "GaBiCategories"}}, {"dataSetInternalID": 10, "referenceToFlowDataSet": {"shortDescription": [{"value": "Nicht-erneuerbare Primärenergie als Energieträger (PENRE)", "lang": "de"}, {"value": "Use of non renewable primary energy (PENRE)", "lang": "en"}, {"value": "Uso de energía primaria no renovable, excluyendo los recursos de energía primaria no renovable utilizada como materia prima (PENRE)", "lang": "es"}, {"value": "Icke förnybar primärenergi - använd som energibärare (PENRE)", "lang": "sv"}], "type": "flow data set", "refObjectId": "ac857178-2b45-46ec-892a-a9a4332f0372", "version": "30.00.002"}, "exchange direction": "INPUT", "meanAmount": 0.0, "other": {"anies": [{"value": "324.655311505081", "module": "A1", "scenario": "Standard scenario"}, {"value": "8.16050157636722", "module": "A2", "scenario": "Standard scenario"}, {"value": "61.8668819627871", "module": "A3", "scenario": "Standard scenario"}, {"value": "394.6826950442353", "module": "A1-A3", "scenario": "Standard scenario"}, {"value": "2.31929647501182", "module": "A4", "scenario": "Standard scenario"}, {"value": "0.149169000257743", "module": "A5", "scenario": "Standard scenario"}, {"value": "7667.99125594347", "module": "B6", "scenario": "Standard scenario"}, {"value": "0.0", "module": "C1", "scenario": "Standard scenario"}, {"value": "0.218064814086049", "module": "C2", "scenario": "Standard scenario"}, {"value": "5.1247026150311", "module": "C3", "scenario": "Standard scenario"}, {"value": "0.010922839257", "module": "C4", "scenario": "Standard scenario"}, {"value": "-46.0463276525764", "module": "D", "scenario": "Standard scenario"}, {"name": "referenceToUnitGroupDataSet", "value": {"shortDescription": [{"value": "MJ"}], "type": "unit group data set", "refObjectId": "93a60a57-a3c8-11da-a746-0800200c9a66", "uri": "../unitgroups/93a60a57-a3c8-11da-a746-0800200c9a66"}}]}, "resolvedFlowVersion": "38.00.000", "flowProperties": [], "typeOfFlow": "Other flow", "classification": {"classHierarchy": "Quantities", "name": "GaBiCategories"}}, {"dataSetInternalID": 11, "referenceToFlowDataSet": {"shortDescription": [{"value": "Nicht-erneuerbare Primärenergie zur stofflichen Nutzung (PENRM)", "lang": "de"}, {"value": "Use of non renewable primary energy resources used as raw materials (PENRM)", "lang": "en"}, {"value": "Uso de la energía primaria no renovable utilizada como materia prima (PENRM)", "lang": "es"}, {"value": "Icke förnybar primärenergi - använd som råmaterial (PENRM)", "lang": "sv"}], "type": "flow data set", "refObjectId": "1421caa0-679d-4bf4-b282-0eb850ccae27", "version": "30.00.001"}, "exchange direction": "INPUT", "meanAmount": 0.0, "other": {"anies": [{"value": "31.6137115299999", "module": "A1", "scenario": "Standard scenario"}, {"value": "0.0", "module": "A2", "scenario": "Standard scenario"}, {"value": "0.3680386439522", "module": "A3", "scenario": "Standard scenario"}, {"value": "31.9817501739521", "module": "A1-A3", "scenario": "Standard scenario"}, {"value": "0.0", "module": "A4", "scenario": "Standard scenario"}, {"value": "0.0", "module": "A5", "scenario": "Standard scenario"}, {"value": "0.0", "module": "B6", "scenario": "Standard scenario"}, {"value": "0.0", "module": "C1", "scenario": "Standard scenario"}, {"value": "0.0", "module": "C2", "scenario": "Standard scenario"}, {"value": "0.0", "module": "C3", "scenario": "Standard scenario"}, {"value": "0.0", "module": "C4", "scenario": "Standard scenario"}, {"value": "-26.4089726038853", "module": "D", "scenario": "Standard scenario"}, {"name": "referenceToUnitGroupDataSet", "value": {"shortDescription": [{"value": "MJ"}], "type": "unit group data set", "refObjectId": "93a60a57-a3c8-11da-a746-0800200c9a66", "uri": "../unitgroups/93a60a57-a3c8-11da-a746-0800200c9a66"}}]}, "resolvedFlowVersion": "38.00.000", "flowProperties": [], "typeOfFlow": "Other flow", "classification": {"classHierarchy": "Quantities", "name": "GaBiCategories"}}, {"dataSetInternalID": 12, "referenceToFlowDataSet": {"shortDescription": [{"value": "Nicht erneuerbare Sekundärbrennstoffe (NRSF)", "lang": "de"}, {"value": "Use of non renewable secondary fuels (NRSF)", "lang": "en"}, {"value": "Uso de combustibles secundarios no renovables (NRSF)", "lang": "es"}, {"value": "Användning av ickeförnybara sekundära bränslen (NRSF)", "lang": "sv"}], "type": "flow data set", "refObjectId": "89def144-d39a-4287-b86f-efde453ddcb2", "version": "30.00.001"}, "exchange direction": "INPUT", "meanAmount": 0.0, "other": {"anies": [{"value": "0.0", "module": "A1", "scenario": "Standard scenario"}, {"value": "0.0", "module": "A2", "scenario": "Standard scenario"}, {"value": "0.0", "module": "A3", "scenario": "Standard scenario"}, {"value": "0.0", "module": "A1-A3", "scenario": "Standard scenario"}, {"value": "0.0", "module": "A4", "scenario": "Standard scenario"}, {"value": "0.0", "module": "A5", "scenario": "Standard scenario"}, {"value": "0.0", "module": "B6", "scenario": "Standard scenario"}, {"value": "0.0", "module": "C1", "scenario": "Standard scenario"}, {"value": "0.0", "module": "C2", "scenario": "Standard scenario"}, {"value": "0.0", "module": "C3", "scenario": "Standard scenario"}, {"value": "0.0", "module": "C4", "scenario": "Standard scenario"}, {"value": "0.0", "module": "D", "scenario": "Standard scenario"}, {"name": "referenceToUnitGroupDataSet", "value": {"shortDescription": [{"value": "MJ"}], "type": "unit group data set", "refObjectId": "93a60a57-a3c8-11da-a746-0800200c9a66", "uri": "../unitgroups/93a60a57-a3c8-11da-a746-0800200c9a66"}}]}, "resolvedFlowVersion": "38.00.000", "flowProperties": [], "typeOfFlow": "Other flow", "classification": {"classHierarchy": "Quantities / Environmental quantities / EPD EN 15804 / LCI indicators", "name": "GaBiCategories"}}, {"dataSetInternalID": 13, "referenceToFlowDataSet": {"shortDescription": [{"value": "Entsorgter radioaktiver Abfall (RWD)", "lang": "de"}, {"value": "Radioactive waste disposed (RWD)", "lang": "en"}, {"value": "Residuos radiactivos eliminados (RWD)", "lang": "es"}, {"value": "Radioaktivt avfall (RWD) ", "lang": "sv"}], "type": "flow data set", "refObjectId": "3449546e-52ad-4b39-b809-9fb77cea8ff6", "version": "30.00.001"}, "exchange direction": "OUTPUT", "meanAmount": 0.0, "other": {"anies": [{"value": "7.569334943954E-4", "module": "A1", "scenario": "Standard scenario"}, {"value": "5.24995054359E-5", "module": "A2", "scenario": "Standard scenario"}, {"value": "3.497603418619E-4", "module": "A3", "scenario": "Standard scenario"}, {"value": "0.0011591933416932", "module": "A1-A3", "scenario": "Standard scenario"}, {"value": "1.43444749648E-5", "module": "A4", "scenario": "Standard scenario"}, {"value": "6.110056566E-7", "module": "A5", "scenario": "Standard scenario"}, {"value": "0.0518594776281698", "module": "B6", "scenario": "Standard scenario"}, {"value": "0.0", "module": "C1", "scenario": "Standard scenario"}, {"value": "1.348695736E-6", "module": "C2", "scenario": "Standard scenario"}, {"value": "1.96475047804E-5", "module": "C3", "scenario": "Standard scenario"}, {"value": "4.60485874E-8", "module": "C4", "scenario": "Standard scenario"}, {"value": "-6.70097212251E-5", "module": "D", "scenario": "Standard scenario"}, {"name": "referenceToUnitGroupDataSet", "value": {"shortDescription": [{"value": "kg"}], "type": "unit group data set", "refObjectId": "ad38d542-3fe9-439d-9b95-2f5f7752acaf", "uri": "../unitgroups/ad38d542-3fe9-439d-9b95-2f5f7752acaf"}}]}, "resolvedFlowVersion": "38.00.000", "flowProperties": [], "typeOfFlow": "Other flow", "classification": {"classHierarchy": "Quantities / Environmental quantities / EPD EN 15804 / LCI indicators", "name": "GaBiCategories"}}, {"dataSetInternalID": 14, "referenceToFlowDataSet": {"shortDescription": [{"value": "Erneuerbare Primärenergie als Energieträger (PERE)", "lang": "de"}, {"value": "Use of renewable primary energy (PERE)", "lang": "en"}, {"value": "Uso de energía primaria renovable excluyendo los recursos de energía primaria renovable utilizada como materia prima (PERE)", "lang": "es"}, {"value": "Förnybar energi - använd som energibärare (PERE)", "lang": "sv"}], "type": "flow data set", "refObjectId": "20f32be5-0398-4288-9b6d-accddd195317", "version": "30.00.001"}, "exchange direction": "INPUT", "meanAmount": 0.0, "other": {"anies": [{"value": "24.1205491140993", "module": "A1", "scenario": "Standard scenario"}, {"value": "0.0841422216670597", "module": "A2", "scenario": "Standard scenario"}, {"value": "7.51782251429999", "module": "A3", "scenario": "Standard scenario"}, {"value": "31.72251385006635", "module": "A1-A3", "scenario": "Standard scenario"}, {"value": "0.0273479109461993", "module": "A4", "scenario": "Standard scenario"}, {"value": "0.0084656971842925", "module": "A5", "scenario": "Standard scenario"}, {"value": "1384.54158309925", "module": "B6", "scenario": "Standard scenario"}, {"value": "0.0", "module": "C1", "scenario": "Standard scenario"}, {"value": "0.0025713043504257", "module": "C2", "scenario": "Standard scenario"}, {"value": "0.32330206279265", "module": "C3", "scenario": "Standard scenario"}, {"value": "6.050582961E-4", "module": "C4", "scenario": "Standard scenario"}, {"value": "-0.337582126198868", "module": "D", "scenario": "Standard scenario"}, {"name": "referenceToUnitGroupDataSet", "value": {"shortDescription": [{"value": "MJ"}], "type": "unit group data set", "refObjectId": "93a60a57-a3c8-11da-a746-0800200c9a66", "uri": "../unitgroups/93a60a57-a3c8-11da-a746-0800200c9a66"}}]}, "resolvedFlowVersion": "38.00.000", "flowProperties": [], "typeOfFlow": "Other flow", "classification": {"classHierarchy": "Quantities", "name": "GaBiCategories"}}, {"dataSetInternalID": 15, "referenceToFlowDataSet": {"shortDescription": [{"value": "Erneuerbare Primärenergie zur stofflichen Nutzung (PERM)", "lang": "de"}, {"value": "Use of renewable primary energy resources used as raw materials (PERM)", "lang": "en"}, {"value": "Uso de energía primaria renovable utilizada como materia prima (PERM)", "lang": "es"}, {"value": "Förnybar energi - använd som råmaterial (PERM)", "lang": "sv"}], "type": "flow data set", "refObjectId": "fb3ec0de-548d-4508-aea5-00b73bf6f702", "version": "30.00.001"}, "exchange direction": "INPUT", "meanAmount": 0.0, "other": {"anies": [{"value": "0.22248648", "module": "A1", "scenario": "Standard scenario"}, {"value": "0.0", "module": "A2", "scenario": "Standard scenario"}, {"value": "6.549608432815", "module": "A3", "scenario": "Standard scenario"}, {"value": "6.772094912815", "module": "A1-A3", "scenario": "Standard scenario"}, {"value": "0.0", "module": "A4", "scenario": "Standard scenario"}, {"value": "0.0", "module": "A5", "scenario": "Standard scenario"}, {"value": "0.0", "module": "B6", "scenario": "Standard scenario"}, {"value": "0.0", "module": "C1", "scenario": "Standard scenario"}, {"value": "0.0", "module": "C2", "scenario": "Standard scenario"}, {"value": "0.0", "module": "C3", "scenario": "Standard scenario"}, {"value": "0.0", "module": "C4", "scenario": "Standard scenario"}, {"value": "-6.9047546", "module": "D", "scenario": "Standard scenario"}, {"name": "referenceToUnitGroupDataSet", "value": {"shortDescription": [{"value": "MJ"}], "type": "unit group data set", "refObjectId": "93a60a57-a3c8-11da-a746-0800200c9a66", "uri": "../unitgroups/93a60a57-a3c8-11da-a746-0800200c9a66"}}]}, "resolvedFlowVersion": "38.00.000", "flowProperties": [], "typeOfFlow": "Other flow", "classification": {"classHierarchy": "Quantities", "name": "GaBiCategories"}}, {"dataSetInternalID": 16, "referenceToFlowDataSet": {"shortDescription": [{"value": "Erneuerbare Sekundärbrennstoffe (RSF)", "lang": "de"}, {"value": "Use of renewable secondary fuels (RSF)", "lang": "en"}, {"value": "Uso de combustibles secundarios renovables (RSF)", "lang": "es"}, {"value": "Användning av förnybara sekundära bränslen (RSF)", "lang": "sv"}], "type": "flow data set", "refObjectId": "64333088-a55f-4aa2-9a31-c10b07816787", "version": "30.00.001"}, "exchange direction": "INPUT", "meanAmount": 0.0, "other": {"anies": [{"value": "0.0", "module": "A1", "scenario": "Standard scenario"}, {"value": "0.0", "module": "A2", "scenario": "Standard scenario"}, {"value": "0.0", "module": "A3", "scenario": "Standard scenario"}, {"value": "0.0", "module": "A1-A3", "scenario": "Standard scenario"}, {"value": "0.0", "module": "A4", "scenario": "Standard scenario"}, {"value": "0.0", "module": "A5", "scenario": "Standard scenario"}, {"value": "0.0", "module": "B6", "scenario": "Standard scenario"}, {"value": "0.0", "module": "C1", "scenario": "Standard scenario"}, {"value": "0.0", "module": "C2", "scenario": "Standard scenario"}, {"value": "0.0", "module": "C3", "scenario": "Standard scenario"}, {"value": "0.0", "module": "C4", "scenario": "Standard scenario"}, {"value": "0.0", "module": "D", "scenario": "Standard scenario"}, {"name": "referenceToUnitGroupDataSet", "value": {"shortDescription": [{"value": "MJ"}], "type": "unit group data set", "refObjectId": "93a60a57-a3c8-11da-a746-0800200c9a66", "uri": "../unitgroups/93a60a57-a3c8-11da-a746-0800200c9a66"}}]}, "resolvedFlowVersion": "38.00.000", "flowProperties": [], "typeOfFlow": "Other flow", "classification": {"classHierarchy": "Quantities / Environmental quantities / EPD EN 15804 / LCI indicators", "name": "GaBiCategories"}}, {"dataSetInternalID": 17, "referenceToFlowDataSet": {"shortDescription": [{"value": "Einsatz von Sekundärstoffen (SM)", "lang": "de"}, {"value": "Use of secondary material (SM)", "lang": "en"}, {"value": "Uso de materiales secundarios (SM)", "lang": "es"}, {"value": "Användning av sekundära material (SM)", "lang": "sv"}], "type": "flow data set", "refObjectId": "c6a1f35f-2d09-4f54-8dfb-97e502e1ce92", "version": "30.00.001"}, "exchange direction": "INPUT", "meanAmount": 0.0, "other": {"anies": [{"value": "0.45146140612834", "module": "A1", "scenario": "Standard scenario"}, {"value": "0.0", "module": "A2", "scenario": "Standard scenario"}, {"value": "0.022573070306417", "module": "A3", "scenario": "Standard scenario"}, {"value": "0.474034476434757", "module": "A1-A3", "scenario": "Standard scenario"}, {"value": "0.0", "module": "A4", "scenario": "Standard scenario"}, {"value": "0.0", "module": "A5", "scenario": "Standard scenario"}, {"value": "0.0", "module": "B6", "scenario": "Standard scenario"}, {"value": "0.0", "module": "C1", "scenario": "Standard scenario"}, {"value": "0.0", "module": "C2", "scenario": "Standard scenario"}, {"value": "0.0", "module": "C3", "scenario": "Standard scenario"}, {"value": "0.0", "module": "C4", "scenario": "Standard scenario"}, {"value": "0.0", "module": "D", "scenario": "Standard scenario"}, {"name": "referenceToUnitGroupDataSet", "value": {"shortDescription": [{"value": "kg"}], "type": "unit group data set", "refObjectId": "ad38d542-3fe9-439d-9b95-2f5f7752acaf", "uri": "../unitgroups/ad38d542-3fe9-439d-9b95-2f5f7752acaf"}}]}, "resolvedFlowVersion": "38.00.000", "flowProperties": [], "typeOfFlow": "Other flow", "classification": {"classHierarchy": "Quantities / Environmental quantities / EPD EN 15804 / LCI indicators", "name": "GaBiCategories"}}, {"dataSetInternalID": 18, "referenceToFlowDataSet": {"shortDescription": [{"value": "Total nicht erneuerbare Primärenergie (PENRT)", "lang": "de"}, {"value": "Total use of non renewable primary energy resource (PENRT)", "lang": "en"}, {"value": "Uso total de la energía primaria no renovable (energía primaria y recursos de energía primaria renovable utilizada como materia prima) (PENRT)", "lang": "es"}, {"value": "Icke förnybar primärenergi – total (PENRT)", "lang": "sv"}], "type": "flow data set", "refObjectId": "06159210-646b-4c8d-8583-da9b3b95a6c1", "version": "30.00.001"}, "exchange direction": "INPUT", "meanAmount": 0.0, "other": {"anies": [{"value": "356.269023035082", "module": "A1", "scenario": "Standard scenario"}, {"value": "8.16050157636722", "module": "A2", "scenario": "Standard scenario"}, {"value": "62.2349923764426", "module": "A3", "scenario": "Standard scenario"}, {"value": "426.66451698789183", "module": "A1-A3", "scenario": "Standard scenario"}, {"value": "2.31929647501182", "module": "A4", "scenario": "Standard scenario"}, {"value": "0.149169000257743", "module": "A5", "scenario": "Standard scenario"}, {"value": "7667.99125594347", "module": "B6", "scenario": "Standard scenario"}, {"value": "0.0", "module": "C1", "scenario": "Standard scenario"}, {"value": "0.218064814086049", "module": "C2", "scenario": "Standard scenario"}, {"value": "5.16662912875645", "module": "C3", "scenario": "Standard scenario"}, {"value": "0.0118682913074682", "module": "C4", "scenario": "Standard scenario"}, {"value": "-72.4462331568914", "module": "D", "scenario": "Standard scenario"}, {"name": "referenceToUnitGroupDataSet", "value": {"shortDescription": [{"value": "MJ"}], "type": "unit group data set", "refObjectId": "93a60a57-a3c8-11da-a746-0800200c9a66", "uri": "../unitgroups/93a60a57-a3c8-11da-a746-0800200c9a66"}}]}, "resolvedFlowVersion": "38.00.000", "flowProperties": [], "typeOfFlow": "Other flow", "classification": {"classHierarchy": "Quantities / Environmental quantities / EPD EN 15804 / LCI indicators", "name": "GaBiCategories"}}, {"dataSetInternalID": 19, "referenceToFlowDataSet": {"shortDescription": [{"value": "Total erneuerbare Primärenergie (PERT)", "lang": "de"}, {"value": "Total use of renewable primary energy resources (PERT)", "lang": "en"}, {"value": "Uso total de la energía primaria renovable (energía primaria y recursos de energía primaria renovable utilizada como materia prima) (PERT)", "lang": "es"}, {"value": "Förnybar energi – total (PERT)", "lang": "sv"}], "type": "flow data set", "refObjectId": "53f97275-fa8a-4cdd-9024-65936002acd0", "version": "30.00.001"}, "exchange direction": "INPUT", "meanAmount": 0.0, "other": {"anies": [{"value": "24.3430355940993", "module": "A1", "scenario": "Standard scenario"}, {"value": "0.0841422216670597", "module": "A2", "scenario": "Standard scenario"}, {"value": "14.0674394896866", "module": "A3", "scenario": "Standard scenario"}, {"value": "38.49461730545296", "module": "A1-A3", "scenario": "Standard scenario"}, {"value": "0.0273479109461993", "module": "A4", "scenario": "Standard scenario"}, {"value": "0.0084656971842925", "module": "A5", "scenario": "Standard scenario"}, {"value": "1384.54158309925", "module": "B6", "scenario": "Standard scenario"}, {"value": "0.0", "module": "C1", "scenario": "Standard scenario"}, {"value": "0.0025713043504257", "module": "C2", "scenario": "Standard scenario"}, {"value": "0.327012670635185", "module": "C3", "scenario": "Standard scenario"}, {"value": "6.216355243874E-4", "module": "C4", "scenario": "Standard scenario"}, {"value": "-7.23955431562602", "module": "D", "scenario": "Standard scenario"}, {"name": "referenceToUnitGroupDataSet", "value": {"shortDescription": [{"value": "MJ"}], "type": "unit group data set", "refObjectId": "93a60a57-a3c8-11da-a746-0800200c9a66", "uri": "../unitgroups/93a60a57-a3c8-11da-a746-0800200c9a66"}}]}, "resolvedFlowVersion": "38.00.000", "flowProperties": [], "typeOfFlow": "Other flow", "classification": {"classHierarchy": "Quantities / Environmental quantities / EPD EN 15804 / LCI indicators", "name": "GaBiCategories"}}]}, "LCIAResults": {"LCIAResult": [{"referenceToLCIAMethodDataSet": {"shortDescription": [{"value": "Potenzial für die Verknappung abiotischer Ressourcen – nicht fossile Ressourcen (ADPE)", "lang": "de"}, {"value": "Abiotic depletion potential - non-fossil resources (ADPE)", "lang": "en"}, {"value": "Abiotisk utarmningspotential icke fossila resurser (ADP-mm)", "lang": "sv"}], "type": "LCIA method data set", "refObjectId": "b2ad6494-c78d-11e6-9d9d-cec0c932ce01", "version": "01.00.013"}, "meanAmount": 0.0, "other": {"anies": [{"value": "0.027620059710713", "module": "A1", "scenario": "Standard scenario"}, {"value": "9.9704306246E-6", "module": "A2", "scenario": "Standard scenario"}, {"value": "2.184000032717E-4", "module": "A3", "scenario": "Standard scenario"}, {"value": "0.0278484301446093", "module": "A1-A3", "scenario": "Standard scenario"}, {"value": "3.669782401E-6", "module": "A4", "scenario": "Standard scenario"}, {"value": "1.965888303E-7", "module": "A5", "scenario": "Standard scenario"}, {"value": "0.0025845739091439", "module": "B6", "scenario": "Standard scenario"}, {"value": "0.0", "module": "C1", "scenario": "Standard scenario"}, {"value": "3.450401558E-7", "module": "C2", "scenario": "Standard scenario"}, {"value": "7.583615875E-6", "module": "C3", "scenario": "Standard scenario"}, {"value": "5.9905301E-9", "module": "C4", "scenario": "Standard scenario"}, {"value": "0.0022904486979214", "module": "D", "scenario": "Standard scenario"}, {"name": "referenceToUnitGroupDataSet", "value": {"shortDescription": [{"value": "kg Sb-Äqv."}], "type": "unit group data set", "refObjectId": "54ccd2d9-a32a-4fc2-923d-f2c8c93e89d4", "uri": "../unitgroups/54ccd2d9-a32a-4fc2-923d-f2c8c93e89d4"}}]}}, {"referenceToLCIAMethodDataSet": {"shortDescription": [{"value": "Potenzial für die Verknappung abiotischer Ressourcen – fossile Brennstoffe (ADPF)", "lang": "de"}, {"value": "Abiotic depletion potential - fossil resources (ADPF)", "lang": "en"}, {"value": "Abiotisk utarmningspotential av fossila resurser (ADP-F)", "lang": "sv"}], "type": "LCIA method data set", "refObjectId": "b2ad6110-c78d-11e6-9d9d-cec0c932ce01", "version": "01.00.012"}, "meanAmount": 0.0, "other": {"anies": [{"value": "332.784099207324", "module": "A1", "scenario": "Standard scenario"}, {"value": "7.68635878536617", "module": "A2", "scenario": "Standard scenario"}, {"value": "58.3401515561375", "module": "A3", "scenario": "Standard scenario"}, {"value": "398.81060954882764", "module": "A1-A3", "scenario": "Standard scenario"}, {"value": "2.18446202732835", "module": "A4", "scenario": "Standard scenario"}, {"value": "0.139871647074822", "module": "A5", "scenario": "Standard scenario"}, {"value": "7308.74244442532", "module": "B6", "scenario": "Standard scenario"}, {"value": "0.0", "module": "C1", "scenario": "Standard scenario"}, {"value": "0.205387414243779", "module": "C2", "scenario": "Standard scenario"}, {"value": "4.84506969338169", "module": "C3", "scenario": "Standard scenario"}, {"value": "0.0111581068165004", "module": "C4", "scenario": "Standard scenario"}, {"value": "-67.687999110499", "module": "D", "scenario": "Standard scenario"}, {"name": "referenceToUnitGroupDataSet", "value": {"shortDescription": [{"value": "MJ"}], "type": "unit group data set", "refObjectId": "93a60a57-a3c8-11da-a746-0800200c9a66", "uri": "../unitgroups/93a60a57-a3c8-11da-a746-0800200c9a66"}}]}}, {"referenceToLCIAMethodDataSet": {"shortDescription": [{"value": "Versauerungspotenzial, kumulierte Überschreitung (AP)", "lang": "de"}, {"value": "Acidification potential, Accumulated Exceedance (AP)", "lang": "en"}, {"value": "Försurningspotential på land och vatten (AP)", "lang": "sv"}], "type": "LCIA method data set", "refObjectId": "b5c611c6-def3-11e6-bf01-fe55135034f3", "version": "01.03.012", "uri": "http://lca.jrc.ec.europa.eu/lcainfohub/datasets/elcd/lciamethods/f6cbd466-253f-4145-a4bb-8dae7d266e89.xml"}, "meanAmount": 0.0, "other": {"anies": [{"value": "0.245369659253952", "module": "A1", "scenario": "Standard scenario"}, {"value": "0.0090494446630012", "module": "A2", "scenario": "Standard scenario"}, {"value": "0.0133323850562374", "module": "A3", "scenario": "Standard scenario"}, {"value": "0.2677514889731906", "module": "A1-A3", "scenario": "Standard scenario"}, {"value": "8.400286651116E-4", "module": "A4", "scenario": "Standard scenario"}, {"value": "1.938049486886E-4", "module": "A5", "scenario": "Standard scenario"}, {"value": "2.07290611257904", "module": "B6", "scenario": "Standard scenario"}, {"value": "0.0", "module": "C1", "scenario": "Standard scenario"}, {"value": "7.89811465063E-5", "module": "C2", "scenario": "Standard scenario"}, {"value": "0.0018503624666034", "module": "C3", "scenario": "Standard scenario"}, {"value": "5.2108387956E-6", "module": "C4", "scenario": "Standard scenario"}, {"value": "-0.0188896644856445", "module": "D", "scenario": "Standard scenario"}, {"name": "referenceToUnitGroupDataSet", "value": {"shortDescription": [{"value": "mol H+ eqv."}], "type": "unit group data set", "refObjectId": "42e089ac-92bf-4bf2-8ca1-5fc40d18f2ed", "uri": "../unitgroups/42e089ac-92bf-4bf2-8ca1-5fc40d18f2ed"}}]}}, {"referenceToLCIAMethodDataSet": {"shortDescription": [{"value": "Eutrophierungspotenzial - Süßwasser (EP-freshwater)", "lang": "de"}, {"value": "Eutrophication potential - freshwater (EP-freshwater)", "lang": "en"}, {"value": "Övergödningspotential sötvatten (EP-fw)", "lang": "sv"}], "type": "LCIA method data set", "refObjectId": "b53ec18f-7377-4ad3-86eb-cc3f4f276b2b", "version": "01.00.012", "uri": "http://lca.jrc.ec.europa.eu/lcainfohub/datasets/elcd/lciamethods/a4630d5b-df2f-48ae-b3f2-5e5257606d68.xml"}, "meanAmount": 0.0, "other": {"anies": [{"value": "0.0081642669205432", "module": "A1", "scenario": "Standard scenario"}, {"value": "3.5888933271E-6", "module": "A2", "scenario": "Standard scenario"}, {"value": "7.18603671878E-5", "module": "A3", "scenario": "Standard scenario"}, {"value": "0.0082397161810581", "module": "A1-A3", "scenario": "Standard scenario"}, {"value": "1.4610841418E-6", "module": "A4", "scenario": "Standard scenario"}, {"value": "3.400150825E-7", "module": "A5", "scenario": "Standard scenario"}, {"value": "0.0379277285739005", "module": "B6", "scenario": "Standard scenario"}, {"value": "0.0", "module": "C1", "scenario": "Standard scenario"}, {"value": "1.373740034E-7", "module": "C2", "scenario": "Standard scenario"}, {"value": "1.12698826748E-5", "module": "C3", "scenario": "Standard scenario"}, {"value": "2.62502502E-8", "module": "C4", "scenario": "Standard scenario"}, {"value": "-1.164550605285E-4", "module": "D", "scenario": "Standard scenario"}, {"name": "referenceToUnitGroupDataSet", "value": {"shortDescription": [{"value": "kg P eqv."}], "type": "unit group data set", "refObjectId": "0429039d-a61d-4590-ba67-aa4a20a810a1", "uri": "../unitgroups/0429039d-a61d-4590-ba67-aa4a20a810a1"}}]}}, {"referenceToLCIAMethodDataSet": {"shortDescription": [{"value": "Eutrophierungspotenzial - Salzwasser (EP-marine)", "lang": "de"}, {"value": "Eutrophication potential - marine (EP-marine)", "lang": "en"}, {"value": "Övergödningspotential marin (EP-m)", "lang": "sv"}], "type": "LCIA method data set", "refObjectId": "b5c619fa-def3-11e6-bf01-fe55135034f3", "version": "02.00.012", "uri": "http://lca.jrc.ec.europa.eu/lcainfohub/datasets/elcd/lciamethods/5296e2be-060b-4e50-b033-d45f85f6ac92.xml"}, "meanAmount": 0.0, "other": {"anies": [{"value": "0.0435431380091723", "module": "A1", "scenario": "Standard scenario"}, {"value": "0.0022444288342334", "module": "A2", "scenario": "Standard scenario"}, {"value": "0.0021767371464806", "module": "A3", "scenario": "Standard scenario"}, {"value": "0.0479643039898863", "module": "A1-A3", "scenario": "Standard scenario"}, {"value": "2.960059569159E-4", "module": "A4", "scenario": "Standard scenario"}, {"value": "8.16174550982E-5", "module": "A5", "scenario": "Standard scenario"}, {"value": "0.26304309772558", "module": "B6", "scenario": "Standard scenario"}, {"value": "0.0", "module": "C1", "scenario": "Standard scenario"}, {"value": "2.78310619874E-5", "module": "C2", "scenario": "Standard scenario"}, {"value": "4.34276438005E-4", "module": "C3", "scenario": "Standard scenario"}, {"value": "2.1546770757E-6", "module": "C4", "scenario": "Standard scenario"}, {"value": "-0.0032660619851265", "module": "D", "scenario": "Standard scenario"}, {"name": "referenceToUnitGroupDataSet", "value": {"shortDescription": [{"value": "kg N eqv."}], "type": "unit group data set", "refObjectId": "d05bb823-ecdf-4686-8c40-bf1d9257859f", "uri": "../unitgroups/d05bb823-ecdf-4686-8c40-bf1d9257859f"}}]}}, {"referenceToLCIAMethodDataSet": {"shortDescription": [{"value": "Eutrophierungspotenzial - Land (EP-terrestrial)", "lang": "de"}, {"value": "Eutrophication potential - terrestrial (EP-terrestrial)", "lang": "en"}, {"value": "Övergödningspotential total (EP-T)", "lang": "sv"}], "type": "LCIA method data set", "refObjectId": "b5c614d2-def3-11e6-bf01-fe55135034f3", "version": "01.02.011", "uri": "http://lca.jrc.ec.europa.eu/lcainfohub/datasets/elcd/lciamethods/40054970-5936-477c-9bec-29fa23b1cb77.xml"}, "meanAmount": 0.0, "other": {"anies": [{"value": "0.531512428515242", "module": "A1", "scenario": "Standard scenario"}, {"value": "0.0249484130346192", "module": "A2", "scenario": "Standard scenario"}, {"value": "0.0244551721737794", "module": "A3", "scenario": "Standard scenario"}, {"value": "0.5809160137236407", "module": "A1-A3", "scenario": "Standard scenario"}, {"value": "0.0032635002452191", "module": "A4", "scenario": "Standard scenario"}, {"value": "9.115559140457E-4", "module": "A5", "scenario": "Standard scenario"}, {"value": "3.24113354810468", "module": "B6", "scenario": "Standard scenario"}, {"value": "0.0", "module": "C1", "scenario": "Standard scenario"}, {"value": "3.068407087713E-4", "module": "C2", "scenario": "Standard scenario"}, {"value": "0.0048502112906139", "module": "C3", "scenario": "Standard scenario"}, {"value": "1.39900116213E-5", "module": "C4", "scenario": "Standard scenario"}, {"value": "-0.034959493746449", "module": "D", "scenario": "Standard scenario"}, {"name": "referenceToUnitGroupDataSet", "value": {"shortDescription": [{"value": "mol N eqv."}], "type": "unit group data set", "refObjectId": "71b4d617-0ec9-4d3f-b65e-e438940c2401", "uri": "../unitgroups/71b4d617-0ec9-4d3f-b65e-e438940c2401"}}]}}, {"referenceToLCIAMethodDataSet": {"shortDescription": [{"value": "Globales Erwärmungspotenzial - total (GWP-total)", "lang": "de"}, {"value": "Global Warming Potential - total (GWP-total)", "lang": "en"}, {"value": "Global uppvärmningspotential – Totalt (GWP-T)", "lang": "sv"}], "type": "LCIA method data set", "refObjectId": "6a37f984-a4b3-458a-a20a-64418c145fa2", "version": "04.00.018"}, "meanAmount": 0.0, "other": {"anies": [{"value": "27.6467330105511", "module": "A1", "scenario": "Standard scenario"}, {"value": "0.546642807317036", "module": "A2", "scenario": "Standard scenario"}, {"value": "3.58252302130129", "module": "A3", "scenario": "Standard scenario"}, {"value": "31.775898839169425", "module": "A1-A3", "scenario": "Standard scenario"}, {"value": "0.144959045810048", "module": "A4", "scenario": "Standard scenario"}, {"value": "0.698983958983377", "module": "A5", "scenario": "Standard scenario"}, {"value": "366.670795779931", "module": "B6", "scenario": "Standard scenario"}, {"value": "0.0", "module": "C1", "scenario": "Standard scenario"}, {"value": "0.01362933446208", "module": "C2", "scenario": "Standard scenario"}, {"value": "0.842175423268033", "module": "C3", "scenario": "Standard scenario"}, {"value": "0.0012227094034756", "module": "C4", "scenario": "Standard scenario"}, {"value": "-3.5238687203049", "module": "D", "scenario": "Standard scenario"}, {"name": "referenceToUnitGroupDataSet", "value": {"shortDescription": [{"value": "kg CO2-Äqv."}], "type": "unit group data set", "refObjectId": "1ebf3012-d0db-4de2-aefd-ef30cedb0be1", "uri": "../unitgroups/1ebf3012-d0db-4de2-aefd-ef30cedb0be1"}}]}}, {"referenceToLCIAMethodDataSet": {"shortDescription": [{"value": "Globales Erwärmungspotenzial - fossil (GWP-fossil)", "lang": "de"}, {"value": "Global Warming Potential - fossil fuels (GWP-fossil)", "lang": "en"}, {"value": "Global uppvärmningspotential– fossil (GWP-f)", "lang": "sv"}], "type": "LCIA method data set", "refObjectId": "5f635281-343e-44fb-83df-1971b155e6b6", "version": "01.00.011"}, "meanAmount": 0.0, "other": {"anies": [{"value": "27.5864704074721", "module": "A1", "scenario": "Standard scenario"}, {"value": "0.546283358441667", "module": "A2", "scenario": "Standard scenario"}, {"value": "4.24795326982247", "module": "A3", "scenario": "Standard scenario"}, {"value": "32.380707035736236", "module": "A1-A3", "scenario": "Standard scenario"}, {"value": "0.144839107080942", "module": "A4", "scenario": "Standard scenario"}, {"value": "0.0125168715128679", "module": "A5", "scenario": "Standard scenario"}, {"value": "355.181931784545", "module": "B6", "scenario": "Standard scenario"}, {"value": "0.0", "module": "C1", "scenario": "Standard scenario"}, {"value": "0.0136180575869819", "module": "C2", "scenario": "Standard scenario"}, {"value": "0.817654652439309", "module": "C3", "scenario": "Standard scenario"}, {"value": "0.001212498839969", "module": "C4", "scenario": "Standard scenario"}, {"value": "-3.52745601207341", "module": "D", "scenario": "Standard scenario"}, {"name": "referenceToUnitGroupDataSet", "value": {"shortDescription": [{"value": "kg CO2-Äqv."}], "type": "unit group data set", "refObjectId": "1ebf3012-d0db-4de2-aefd-ef30cedb0be1", "uri": "../unitgroups/1ebf3012-d0db-4de2-aefd-ef30cedb0be1"}}]}}, {"referenceToLCIAMethodDataSet": {"shortDescription": [{"value": "Globales Erwärmungspotenzial - biogen (GWP-biogenic)", "lang": "de"}, {"value": "Global Warming Potential - biogenic (GWP-biogenic)", "lang": "en"}, {"value": "Global uppvärmningspotential – biogen (GWP-b)", "lang": "sv"}], "type": "LCIA method data set", "refObjectId": "2356e1ab-0185-4db5-86e5-16de51c7485c", "version": "01.00.007"}, "meanAmount": 0.0, "other": {"anies": [{"value": "0.0246225616664803", "module": "A1", "scenario": "Standard scenario"}, {"value": "8.23171206611E-5", "module": "A2", "scenario": "Standard scenario"}, {"value": "-0.672082190625777", "module": "A3", "scenario": "Standard scenario"}, {"value": "-0.6473773118386356", "module": "A1-A3", "scenario": "Standard scenario"}, {"value": "6.68647971515E-5", "module": "A4", "scenario": "Standard scenario"}, {"value": "0.68645890393862", "module": "A5", "scenario": "Standard scenario"}, {"value": "10.6628584028714", "module": "B6", "scenario": "Standard scenario"}, {"value": "0.0", "module": "C1", "scenario": "Standard scenario"}, {"value": "6.2867596777E-6", "module": "C2", "scenario": "Standard scenario"}, {"value": "0.0242209517415721", "module": "C3", "scenario": "Standard scenario"}, {"value": "9.5166696404E-6", "module": "C4", "scenario": "Standard scenario"}, {"value": "0.0147499676742804", "module": "D", "scenario": "Standard scenario"}, {"name": "referenceToUnitGroupDataSet", "value": {"shortDescription": [{"value": "kg CO2-Äqv."}], "type": "unit group data set", "refObjectId": "1ebf3012-d0db-4de2-aefd-ef30cedb0be1", "uri": "../unitgroups/1ebf3012-d0db-4de2-aefd-ef30cedb0be1"}}]}}, {"referenceToLCIAMethodDataSet": {"shortDescription": [{"value": "Globales Erwärmungspotenzial - luluc (GWP-luluc)", "lang": "de"}, {"value": "Global Warming Potential - land use and land use change (GWP-luluc)", "lang": "en"}, {"value": "Global uppvärmningspotential - markanvändning och förändringar i markanvändning (GWP-luluc)", "lang": "sv"}], "type": "LCIA method data set", "refObjectId": "4331bbdb-978a-490d-8707-eeb047f01a55", "version": "01.00.007"}, "meanAmount": 0.0, "other": {"anies": [{"value": "0.0356401536677738", "module": "A1", "scenario": "Standard scenario"}, {"value": "2.771317547094E-4", "module": "A2", "scenario": "Standard scenario"}, {"value": "0.0066520858574644", "module": "A3", "scenario": "Standard scenario"}, {"value": "0.0425693712799476", "module": "A1-A3", "scenario": "Standard scenario"}, {"value": "5.30739319548E-5", "module": "A4", "scenario": "Standard scenario"}, {"value": "8.3914118893E-6", "module": "A5", "scenario": "Standard scenario"}, {"value": "0.826005592514571", "module": "B6", "scenario": "Standard scenario"}, {"value": "0.0", "module": "C1", "scenario": "Standard scenario"}, {"value": "4.9901154204E-6", "module": "C2", "scenario": "Standard scenario"}, {"value": "3.031716559281E-4", "module": "C3", "scenario": "Standard scenario"}, {"value": "6.957955067E-7", "module": "C4", "scenario": "Standard scenario"}, {"value": "-0.011163480607539", "module": "D", "scenario": "Standard scenario"}, {"name": "referenceToUnitGroupDataSet", "value": {"shortDescription": [{"value": "kg CO2-Äqv."}], "type": "unit group data set", "refObjectId": "1ebf3012-d0db-4de2-aefd-ef30cedb0be1", "uri": "../unitgroups/1ebf3012-d0db-4de2-aefd-ef30cedb0be1"}}]}}, {"referenceToLCIAMethodDataSet": {"shortDescription": [{"value": "Abbaupotenzial der stratosphärischen Ozonschicht (ODP)", "lang": "de"}, {"value": "Depletion potential of the stratospheric ozone layer (ODP)", "lang": "en"}, {"value": "Utarmningspotential för stratosfäriska ozonskiktet - ozonnedbrytning (ODP)", "lang": "sv"}], "type": "LCIA method data set", "refObjectId": "b5c629d6-def3-11e6-bf01-fe55135034f3", "version": "02.00.014", "uri": "http://lca.jrc.ec.europa.eu/lcainfohub/datasets/elcd/lciamethods/8b723200-3d8f-4eec-9e10-444edb029476.xml"}, "meanAmount": 0.0, "other": {"anies": [{"value": "1.3833655804E-6", "module": "A1", "scenario": "Standard scenario"}, {"value": "1.171679576E-7", "module": "A2", "scenario": "Standard scenario"}, {"value": "7.480398306E-7", "module": "A3", "scenario": "Standard scenario"}, {"value": "2.2485733686E-6", "module": "A1-A3", "scenario": "Standard scenario"}, {"value": "3.19694695E-8", "module": "A4", "scenario": "Standard scenario"}, {"value": "3.6210467E-9", "module": "A5", "scenario": "Standard scenario"}, {"value": "2.99116155098E-5", "module": "B6", "scenario": "Standard scenario"}, {"value": "0.0", "module": "C1", "scenario": "Standard scenario"}, {"value": "3.0058324E-9", "module": "C2", "scenario": "Standard scenario"}, {"value": "4.42869897E-8", "module": "C3", "scenario": "Standard scenario"}, {"value": "9.39046E-11", "module": "C4", "scenario": "Standard scenario"}, {"value": "-1.387342964E-7", "module": "D", "scenario": "Standard scenario"}, {"name": "referenceToUnitGroupDataSet", "value": {"shortDescription": [{"value": "kg CFC 11-Äquiv."}], "type": "unit group data set", "refObjectId": "d9e957c9-7309-4474-bf3a-7777df6c4e5b", "uri": "../unitgroups/d9e957c9-7309-4474-bf3a-7777df6c4e5b"}}]}}, {"referenceToLCIAMethodDataSet": {"shortDescription": [{"value": "Bildungspotenzial für troposphärisches Ozon (POCP)", "lang": "de"}, {"value": "Photochemical Ozone Creation Potential (POCP)", "lang": "en"}, {"value": "Potential till fotokemisk oxidantbildning – marknära ozon (POCP)", "lang": "sv"}], "type": "LCIA method data set", "refObjectId": "b5c610fe-def3-11e6-bf01-fe55135034f3", "version": "02.00.018", "uri": "http://lca.jrc.ec.europa.eu/lcainfohub/datasets/elcd/lciamethods/ec7836be-83eb-41da-bcda-1a6a3fe2d149.xml"}, "meanAmount": 0.0, "other": {"anies": [{"value": "0.14224154737518", "module": "A1", "scenario": "Standard scenario"}, {"value": "0.0066853886123247", "module": "A2", "scenario": "Standard scenario"}, {"value": "0.0076285737229036", "module": "A3", "scenario": "Standard scenario"}, {"value": "0.1565555097104083", "module": "A1-A3", "scenario": "Standard scenario"}, {"value": "9.317528243376E-4", "module": "A4", "scenario": "Standard scenario"}, {"value": "2.36331220173E-4", "module": "A5", "scenario": "Standard scenario"}, {"value": "0.822444891639105", "module": "B6", "scenario": "Standard scenario"}, {"value": "0.0", "module": "C1", "scenario": "Standard scenario"}, {"value": "8.76052322773E-5", "module": "C2", "scenario": "Standard scenario"}, {"value": "0.001482774713616", "module": "C3", "scenario": "Standard scenario"}, {"value": "4.2358715566E-6", "module": "C4", "scenario": "Standard scenario"}, {"value": "-0.0114763415120529", "module": "D", "scenario": "Standard scenario"}, {"name": "referenceToUnitGroupDataSet", "value": {"shortDescription": [{"value": "kg NMVOC eqv."}], "type": "unit group data set", "refObjectId": "d27c25f8-fbc1-44c6-b47b-4adbae4199c6", "uri": "../unitgroups/d27c25f8-fbc1-44c6-b47b-4adbae4199c6"}}]}}, {"referenceToLCIAMethodDataSet": {"shortDescription": [{"value": "Wasser-Entzugspotenzial (Benutzer) (WDP)", "lang": "de"}, {"value": "Water (user) deprivation potential (WDP)", "lang": "en"}, {"value": "Vattenfotavtryck (WDP)", "lang": "sv"}], "type": "LCIA method data set", "refObjectId": "b2ad66ce-c78d-11e6-9d9d-cec0c932ce01", "version": "03.00.016"}, "meanAmount": 0.0, "other": {"anies": [{"value": "6.94928420234383", "module": "A1", "scenario": "Standard scenario"}, {"value": "0.018419181200369", "module": "A2", "scenario": "Standard scenario"}, {"value": "0.33908095011116", "module": "A3", "scenario": "Standard scenario"}, {"value": "7.30678433365536", "module": "A1-A3", "scenario": "Standard scenario"}, {"value": "0.0078153384007205", "module": "A4", "scenario": "Standard scenario"}, {"value": "0.0056035194225702", "module": "A5", "scenario": "Standard scenario"}, {"value": "81.8635756281324", "module": "B6", "scenario": "Standard scenario"}, {"value": "0.0", "module": "C1", "scenario": "Standard scenario"}, {"value": "7.348134806112E-4", "module": "C2", "scenario": "Standard scenario"}, {"value": "0.0903849752370723", "module": "C3", "scenario": "Standard scenario"}, {"value": "3.011964070561E-4", "module": "C4", "scenario": "Standard scenario"}, {"value": "-0.933699401171686", "module": "D", "scenario": "Standard scenario"}, {"name": "referenceToUnitGroupDataSet", "value": {"shortDescription": [{"value": "m3 world eqv."}], "type": "unit group data set", "refObjectId": "6ae2df01-888e-46c8-b17d-49fa3869b476", "uri": "../unitgroups/6ae2df01-888e-46c8-b17d-49fa3869b476"}}]}}, {"referenceToLCIAMethodDataSet": {"shortDescription": [{"value": "Potenzielles Auftreten von Krankheiten aufgrund von Feinstaubemissionen (PM)", "lang": "de"}, {"value": "Potential incidence of disease due to PM emissions (PM)", "lang": "en"}, {"value": "Potential till utsläpp av partiklar (PM)", "lang": "sv"}], "type": "LCIA method data set", "refObjectId": "b5c602c6-def3-11e6-bf01-fe55135034f3", "version": "02.00.013", "uri": "http://lca.jrc.ec.europa.eu/lcainfohub/datasets/elcd/lciamethods/72ce3013-f678-4c6a-935b-f4752ff8901b.xml"}, "meanAmount": 0.0, "other": {"anies": [{"value": "1.886982153E-6", "module": "A1", "scenario": "Standard scenario"}, {"value": "2.89322822E-8", "module": "A2", "scenario": "Standard scenario"}, {"value": "1.154776215E-7", "module": "A3", "scenario": "Standard scenario"}, {"value": "2.0313920567000004E-6", "module": "A1-A3", "scenario": "Standard scenario"}, {"value": "1.30302461E-8", "module": "A4", "scenario": "Standard scenario"}, {"value": "1.5784893E-9", "module": "A5", "scenario": "Standard scenario"}, {"value": "5.427116372E-6", "module": "B6", "scenario": "Standard scenario"}, {"value": "0.0", "module": "C1", "scenario": "Standard scenario"}, {"value": "1.2251294E-9", "module": "C2", "scenario": "Standard scenario"}, {"value": "2.70417241E-8", "module": "C3", "scenario": "Standard scenario"}, {"value": "7.25164E-11", "module": "C4", "scenario": "Standard scenario"}, {"value": "-2.26198628E-7", "module": "D", "scenario": "Standard scenario"}, {"name": "referenceToUnitGroupDataSet", "value": {"shortDescription": [{"value": "disease incidence"}], "type": "unit group data set", "refObjectId": "3883559b-648f-4afc-8ba2-0bd24f3affa3", "uri": "../unitgroups/3883559b-648f-4afc-8ba2-0bd24f3affa3"}}]}}, {"referenceToLCIAMethodDataSet": {"shortDescription": [{"value": "Potenzielle Wirkung durch Exposition des Menschen mit U235 (IRP)", "lang": "de"}, {"value": "Potential Human exposure efficiency relative to U235 (IRP)", "lang": "en"}, {"value": "Exponeringseffektivitet relaterad till U235 (IR)", "lang": "sv"}], "type": "LCIA method data set", "refObjectId": "b5c632be-def3-11e6-bf01-fe55135034f3", "version": "01.00.013", "uri": "http://lca.jrc.ec.europa.eu/lcainfohub/datasets/elcd/lciamethods/a6f4cbc8-5388-44d6-9a67-53d05684f93e.xml"}, "meanAmount": 0.0, "other": {"anies": [{"value": "1.11679069664392", "module": "A1", "scenario": "Standard scenario"}, {"value": "0.0331172715589871", "module": "A2", "scenario": "Standard scenario"}, {"value": "0.247244088014146", "module": "A3", "scenario": "Standard scenario"}, {"value": "1.3971520562170532", "module": "A1-A3", "scenario": "Standard scenario"}, {"value": "0.0091525766046031", "module": "A4", "scenario": "Standard scenario"}, {"value": "5.265073649347E-4", "module": "A5", "scenario": "Standard scenario"}, {"value": "63.1561593362579", "module": "B6", "scenario": "Standard scenario"}, {"value": "0.0", "module": "C1", "scenario": "Standard scenario"}, {"value": "8.605432454171E-4", "module": "C2", "scenario": "Standard scenario"}, {"value": "0.0164394127710325", "module": "C3", "scenario": "Standard scenario"}, {"value": "3.83664752109E-5", "module": "C4", "scenario": "Standard scenario"}, {"value": "-0.0623320416135083", "module": "D", "scenario": "Standard scenario"}, {"name": "referenceToUnitGroupDataSet", "value": {"shortDescription": [{"value": "kBq U235 eqv."}], "type": "unit group data set", "refObjectId": "456b05bf-1415-44a9-9993-02452f554c09", "uri": "../unitgroups/456b05bf-1415-44a9-9993-02452f554c09"}}]}}, {"referenceToLCIAMethodDataSet": {"shortDescription": [{"value": "Potenzielle Toxizitätsvergleichseinheit für Ökosysteme (ETP-fw)", "lang": "de"}, {"value": "Potential Comparative Toxic Unit for ecosystems (ETP-fw)", "lang": "en"}, {"value": "Ecotoxicitet (ETP-fw) ", "lang": "sv"}], "type": "LCIA method data set", "refObjectId": "ee1082d1-b0f7-43ca-a1f0-21e2a4a74511", "version": "01.00.004", "uri": "http://lca.jrc.ec.europa.eu/lcainfohub/datasets/elcd/lciamethods/ee1082d1-b0f7-43ca-a1f0-21e2a4a74511.xml"}, "meanAmount": 0.0, "other": {"anies": [{"value": "3690.67307223999", "module": "A1", "scenario": "Standard scenario"}, {"value": "5.7953286116368", "module": "A2", "scenario": "Standard scenario"}, {"value": "54.5640806951857", "module": "A3", "scenario": "Standard scenario"}, {"value": "3751.032481546812", "module": "A1-A3", "scenario": "Standard scenario"}, {"value": "1.94793093820465", "module": "A4", "scenario": "Standard scenario"}, {"value": "1.08910747273053", "module": "A5", "scenario": "Standard scenario"}, {"value": "5004.4124411166", "module": "B6", "scenario": "Standard scenario"}, {"value": "0.0", "module": "C1", "scenario": "Standard scenario"}, {"value": "0.18314829624785", "module": "C2", "scenario": "Standard scenario"}, {"value": "11.3234327268014", "module": "C3", "scenario": "Standard scenario"}, {"value": "11.295542597923", "module": "C4", "scenario": "Standard scenario"}, {"value": "-89.9815792239822", "module": "D", "scenario": "Standard scenario"}, {"name": "referenceToUnitGroupDataSet", "value": {"shortDescription": [{"value": "CTUe"}], "type": "unit group data set", "refObjectId": "aa959ded-f1eb-4efb-9c5c-2d60be36b3e6", "uri": "../unitgroups/aa959ded-f1eb-4efb-9c5c-2d60be36b3e6"}}]}}, {"referenceToLCIAMethodDataSet": {"shortDescription": [{"value": "Potenzielle Toxizitätsvergleichseinheit für den Menschen - kanzerogene Wirkung (HTP-c)", "lang": "de"}, {"value": "Potential Comparative Toxic Unit for humans - cancer effects (HTP-c)", "lang": "en"}, {"value": "Humantoxicitet – cancer (HTP-c)", "lang": "sv"}], "type": "LCIA method data set", "refObjectId": "2299222a-bbd8-474f-9d4f-4dd1f18aea7c", "version": "01.00.005", "uri": "http://lca.jrc.ec.europa.eu/lcainfohub/datasets/elcd/lciamethods/2299222a-bbd8-474f-9d4f-4dd1f18aea7c.xml"}, "meanAmount": 0.0, "other": {"anies": [{"value": "1.99056848E-8", "module": "A1", "scenario": "Standard scenario"}, {"value": "2.487701E-10", "module": "A2", "scenario": "Standard scenario"}, {"value": "1.0519267E-9", "module": "A3", "scenario": "Standard scenario"}, {"value": "2.1206381599999997E-8", "module": "A1-A3", "scenario": "Standard scenario"}, {"value": "6.318E-11", "module": "A4", "scenario": "Standard scenario"}, {"value": "1.444188E-10", "module": "A5", "scenario": "Standard scenario"}, {"value": "1.292168989E-7", "module": "B6", "scenario": "Standard scenario"}, {"value": "0.0", "module": "C1", "scenario": "Standard scenario"}, {"value": "5.9403E-12", "module": "C2", "scenario": "Standard scenario"}, {"value": "5.129078E-10", "module": "C3", "scenario": "Standard scenario"}, {"value": "6.734E-13", "module": "C4", "scenario": "Standard scenario"}, {"value": "-2.9309999E-9", "module": "D", "scenario": "Standard scenario"}, {"name": "referenceToUnitGroupDataSet", "value": {"shortDescription": [{"value": "CTUh"}], "type": "unit group data set", "refObjectId": "d4c9523e-2d7e-49fd-8469-998f547d3a70", "uri": "../unitgroups/d4c9523e-2d7e-49fd-8469-998f547d3a70"}}]}}, {"referenceToLCIAMethodDataSet": {"shortDescription": [{"value": "Potenzielle Toxizitätsvergleichseinheit für den Menschen - nicht kanzerogene Wirkung (HTP-nc)", "lang": "de"}, {"value": "Potential Comparative Toxic Unit for humans - non-cancer effects (HTP-nc)", "lang": "en"}, {"value": "Humantoxicitet – icke cancer (HTP-nc)", "lang": "sv"}], "type": "LCIA method data set", "refObjectId": "3af763a5-b7a1-48c9-9cee-1f223481fcef", "version": "01.00.004", "uri": "http://lca.jrc.ec.europa.eu/lcainfohub/datasets/elcd/lciamethods/3af763a5-b7a1-48c9-9cee-1f223481fcef.xml"}, "meanAmount": 0.0, "other": {"anies": [{"value": "8.869065476E-7", "module": "A1", "scenario": "Standard scenario"}, {"value": "5.6395977E-9", "module": "A2", "scenario": "Standard scenario"}, {"value": "3.09367756E-8", "module": "A3", "scenario": "Standard scenario"}, {"value": "9.234829208999999E-7", "module": "A1-A3", "scenario": "Standard scenario"}, {"value": "2.1307437E-9", "module": "A4", "scenario": "Standard scenario"}, {"value": "1.0158072E-9", "module": "A5", "scenario": "Standard scenario"}, {"value": "4.406218809E-6", "module": "B6", "scenario": "Standard scenario"}, {"value": "0.0", "module": "C1", "scenario": "Standard scenario"}, {"value": "2.003367E-10", "module": "C2", "scenario": "Standard scenario"}, {"value": "1.17317912E-8", "module": "C3", "scenario": "Standard scenario"}, {"value": "1.94359E-11", "module": "C4", "scenario": "Standard scenario"}, {"value": "-4.22864353E-8", "module": "D", "scenario": "Standard scenario"}, {"name": "referenceToUnitGroupDataSet", "value": {"shortDescription": [{"value": "CTUh"}], "type": "unit group data set", "refObjectId": "d4c9523e-2d7e-49fd-8469-998f547d3a70", "uri": "../unitgroups/d4c9523e-2d7e-49fd-8469-998f547d3a70"}}]}}, {"referenceToLCIAMethodDataSet": {"shortDescription": [{"value": "Potenzieller Bodenqualitätsindex (SQP)", "lang": "de"}, {"value": "Potential Soil quality index (SQP)", "lang": "en"}, {"value": "Potentiell jordkvalitet index (SQP)", "lang": "sv"}], "type": "LCIA method data set", "refObjectId": "b2ad6890-c78d-11e6-9d9d-cec0c932ce01", "version": "01.00.014"}, "meanAmount": 0.0, "other": {"anies": [{"value": "140.221320532633", "module": "A1", "scenario": "Standard scenario"}, {"value": "3.82550265187901", "module": "A2", "scenario": "Standard scenario"}, {"value": "71.7943276250212", "module": "A3", "scenario": "Standard scenario"}, {"value": "215.84115080953322", "module": "A1-A3", "scenario": "Standard scenario"}, {"value": "1.8944579151096", "module": "A4", "scenario": "Standard scenario"}, {"value": "0.0680048186633279", "module": "A5", "scenario": "Standard scenario"}, {"value": "1784.74131971432", "module": "B6", "scenario": "Standard scenario"}, {"value": "0.0", "module": "C1", "scenario": "Standard scenario"}, {"value": "0.178120657493827", "module": "C2", "scenario": "Standard scenario"}, {"value": "4.00511666504427", "module": "C3", "scenario": "Standard scenario"}, {"value": "0.0148777821424446", "module": "C4", "scenario": "Standard scenario"}, {"value": "-22.4115630810743", "module": "D", "scenario": "Standard scenario"}, {"name": "referenceToUnitGroupDataSet", "value": {"shortDescription": [{"value": "dimensionless"}], "type": "unit group data set", "refObjectId": "f130951c-e67f-4f7f-8dd4-665de3974e18", "uri": "../unitgroups/f130951c-e67f-4f7f-8dd4-665de3974e18"}}]}}]}, "otherAttributes": {"{http://www.okworx.com/ILCD/Extensions/2018/Profile}profile": "EN_15804_A2", "{http://www.indata.network/EPD/2019}epd-version": "1.2"}, "version": "1.1"}