{"processInformation": {"dataSetInformation": {"UUID": "129f826b-d300-47ca-b81f-69dd1372496b", "name": {"baseName": [{"value": "PROMATECT®–H", "lang": "en"}, {"value": "PROMATECT®-H", "lang": "de"}], "functionalUnitFlowProperties": [{"lang": "en"}]}, "classificationInformation": {"classification": [{"class": [{"value": "Dämmstoffe", "level": 0, "classId": "2"}, {"value": "Calciumsilikat / Calcium-Silikathydrat", "level": 1, "classId": "2.20"}, {"value": "Calciumsilikat", "level": 2, "classId": "2.20.02"}], "name": "OEKOBAU.DAT"}, {"class": [{"value": "02 Building products", "level": 0}, {"value": "Thermal insulation products", "level": 1}, {"value": "Calcium silicate insulating materials", "level": 2}], "name": "IBUCategories"}]}, "generalComment": [{"value": "PROMATECT®–H is a fire-protective cement bonded calcium silicate based insulation board and is asbestos free. This large-sized multi-purpose board is easy to handle and offers a combination of enhanced mechanical properties for self-supporting constructions. PROMATECT®–H is hygroscopic and vapour permeable. Moisture content is therefore automatically regulated by the application environment.", "lang": "en"}, {"value": "PROMATECT®-H ist eine zementgebundene Brandschutzdämmplatte auf Kalziumsilikatbasis und ist asbestfrei. Diese großformatige Mehrzweckplatte ist leicht zu verarbeiten und bietet eine Kombination aus verbesserten mechanischen Eigenschaften für selbsttragende Konstruktionen. PROMATECT®-H ist hygroskopisch und dampfdurchlässig. Der Feuchtigkeitsgehalt wird daher automatisch durch die Anwendungsumgebung reguliert.", "lang": "de"}], "other": {"anies": [{"scenario": [{"description": [{"value": "100% recycling", "lang": "en"}, {"value": "100% Recycling", "lang": "de"}], "name": "S1", "default": true}, {"description": [{"value": "100% landfill", "lang": "en"}, {"value": "100% Deponie", "lang": "de"}], "name": "S2"}]}]}}, "quantitativeReference": {"referenceToReferenceFlow": [0]}, "time": {"referenceYear": 2023, "dataSetValidUntil": 2028, "other": {"anies": [{"name": "publicationDateOfEPD", "value": 1690761600000}]}}, "geography": {"locationOfOperationSupplyOrProduction": {"location": "CN"}}, "technology": {"technologyDescriptionAndIncludedProcesses": [{"value": "All the raw materials are mixed in water and combined to form a thick slurry. The slurry is formed to a board on a forming drum, cut and stacked for curing. The board is autoclaved under saturated steam pressure and dried. Edges are trimmed and the reverse surface sanded to the desired thickness. All material which is cut off or sanded away is fully recycled within the process. \nDeclared unit: \nProduction and installation of 1 m2 of PROMATECT®–H with a thickness of 20 mm", "lang": "en"}, {"value": "Alle Rohstoffe werden mit Wasser vermischt und zu einem dicken Brei verarbeitet. Die Aufschlämmung wird auf einer Formtrommel zu einer Platte geformt, geschnitten und zum Aushärten gestapelt. Die Platte wird unter gesättigtem Dampfdruck autoklaviert und getrocknet. Die Kanten werden abgeschnitten und die Rückseite auf die gewünschte Dicke geschliffen. Das gesamte abgeschnittene oder weggeschliffene Material wird im Prozess vollständig wiederverwertet. \nTechnische Daten: \n siehe pdf tabelle der technischen daten \nDeklarierte Einheit: \nHerstellung und Verlegung von 1 m2 PROMATECT®-H mit einer Dicke von 20 mm", "lang": "de"}], "technologicalApplicability": [{"value": "Promat fire protection boards:\nStructural steel protection\nConcrete floor and wall upgrading\nM&E services enclosure\nAccess panels and hatches, fire doors\nMembrane ceilings\nCladding to steel ducts, self-supporting ductsIn some applications the boards are installed on a substructure.\nNote that the substructure is not included in the scope of the EPD.", "lang": "en"}, {"value": "Promat-Brandschutzplatten: Schutz von Stahlkonstruktionen Ausbau von Betonböden und -wänden Umhüllung von Haustechnik Zugangspaneele und Luken, Brandschutztüren Membrandecken Verkleidung von Stahlkanälen, selbsttragende KanäleIn einigen Fällen werden die Platten auf einer Unterkonstruktion montiert. Beachten Sie, dass die Unterkonstruktion nicht zum Umfang der EPD gehört.", "lang": "de"}]}}, "modellingAndValidation": {"LCIMethodAndAllocation": {"typeOfDataSet": "EPD", "referenceToLCAMethodDetails": [{"shortDescription": [{"value": "Calcium silicate insulating materials.pdf", "lang": "en"}], "type": "source data set", "refObjectId": "5606c57c-bb4c-4d2c-8d36-3907a011b7a5"}], "other": {"anies": [{"name": "subType", "value": "specific dataset"}]}}, "dataSourcesTreatmentAndRepresentativeness": {"referenceToDataSource": [{"shortDescription": [{"value": "ecoinvent database (all versions)", "lang": "en"}], "type": "source data set", "refObjectId": "b497a91f-e14b-4b69-8f28-f50eb1576766"}, {"shortDescription": [{"value": "ecoinvent 3.8 database", "lang": "en"}], "type": "source data set", "refObjectId": "0f4c65c0-6210-450f-b886-82bf8dd5ace9"}], "useAdviceForDataSet": [{"value": "Scope: \nThis EPD is representative and relevant for PROMATECT®–H boards produced by ETEX in Guangzhou (China) and installed in Europe. The data describing the direct inputs and outputs of the foreground processes are representative for ETEX production of the year 2021 in Guangzhou, China. \nSystem boundary: \nCradle-to-grave", "lang": "en"}, {"value": "Gültigkeitsbereich: \nDiese EPD ist repräsentativ und relevant für PROMATECT®-H Platten, die von ETEX in Guangzhou (China) produziert und in Europa installiert werden. Die Daten, die die direkten Inputs und Outputs der Vordergrundprozesse beschreiben, sind repräsentativ für die ETEX-Produktion des Jahres 2021 in Guangzhou, China. \nSystemgrenze: \nVon der Wiege bis zur Bahre", "lang": "de"}], "other": {"anies": [{"name": "referenceToOriginalEPD", "value": {"shortDescription": {"value": "PROMATECT®–H.pdf", "defaultValue": "PROMATECT®–H.pdf", "lstrings": [{"lang": "en", "value": "PROMATECT®–H.pdf"}]}, "type": "source data set", "uuid": {"uuid": "e3691c7d-e422-4229-867f-cc42db51e301"}, "refObjectId": "e3691c7d-e422-4229-867f-cc42db51e301", "resourceURLs": ["https://oekobaudat.de/OEKOBAU.DAT/resource/sources/e3691c7d-e422-4229-867f-cc42db51e301/PROMATECTH_18597.pdf?version=00.02.000"]}}]}}, "validation": {"review": [{"referenceToNameOfReviewerAndInstitution": [{"shortDescription": [{"value": "Institut Bauen und Umwelt e. V.", "lang": "en"}], "type": "contact data set", "refObjectId": "d111dbec-b024-4be5-86c5-752d6eb2cf95", "uri": "../contacts/d111dbec-b024-4be5-86c5-752d6eb2cf95.xml"}], "type": "Accredited third party review"}]}, "complianceDeclarations": {"compliance": [{"referenceToComplianceSystem": {"shortDescription": [{"value": "DIN EN 15804+A2", "lang": "en"}], "type": "source data set", "refObjectId": "c0016b33-8cf7-415c-ac6e-deba0d21440d", "uri": "../sources/c0016b33-8cf7-415c-ac6e-deba0d21440d.xml"}}, {"referenceToComplianceSystem": {"shortDescription": [{"value": "ISO 14025", "lang": "en"}], "type": "source data set", "refObjectId": "4f2eb655-6e44-4874-a95a-e28f5442cd4d", "uri": "../sources/4f2eb655-6e44-4874-a95a-e28f5442cd4d.xml"}}]}}, "administrativeInformation": {"commissionerAndGoal": {"referenceToCommissioner": [{"shortDescription": [{"value": "Etex Building Performance International", "lang": "en"}], "type": "contact data set", "refObjectId": "9f15c029-1fb0-467d-8dd1-92b013e91ca8", "uri": "../contacts/9f15c029-1fb0-467d-8dd1-92b013e91ca8.xml"}]}, "dataGenerator": {"referenceToPersonOrEntityGeneratingTheDataSet": [{"shortDescription": [{"value": "Enperas", "lang": "en"}], "type": "contact data set", "refObjectId": "71c3ddb3-f20b-4161-af33-52bc33b3106d", "uri": "../contacts/71c3ddb3-f20b-4161-af33-52bc33b3106d.xml"}]}, "dataEntryBy": {"timeStamp": 1690761600000, "referenceToDataSetFormat": [{"shortDescription": [{"value": "ILCD Format", "lang": "en"}], "type": "source data set", "refObjectId": "a97a0155-0234-4b87-b4ce-a45da52f2a40", "uri": "../sources/a97a0155-0234-4b87-b4ce-a45da52f2a40.xml"}, {"shortDescription": [{"value": "EPD-Datenformaterweiterungen v1.2", "lang": "de"}, {"value": "EPD Data Format Extensions v1.2", "lang": "en"}], "type": "source data set", "refObjectId": "a29449fd-aa2f-4de8-b5d7-4b06b43c6fde", "uri": "../sources/a29449fd-aa2f-4de8-b5d7-4b06b43c6fde.xml"}]}, "publicationAndOwnership": {"dataSetVersion": "00.07.000", "referenceToRegistrationAuthority": {"shortDescription": [{"value": "Institut Bauen und Umwelt e. V.", "lang": "en"}], "type": "contact data set", "refObjectId": "d111dbec-b024-4be5-86c5-752d6eb2cf95", "uri": "../contacts/d111dbec-b024-4be5-86c5-752d6eb2cf95.xml"}, "registrationNumber": "EPD-ETE-20230130-IBA2-EN", "referenceToOwnershipOfDataSet": {"shortDescription": [{"value": "Etex Building Performance International", "lang": "en"}], "type": "contact data set", "refObjectId": "9f15c029-1fb0-467d-8dd1-92b013e91ca8", "uri": "../contacts/9f15c029-1fb0-467d-8dd1-92b013e91ca8.xml"}, "copyright": true, "licenseType": "Free of charge for all users and uses", "accessRestrictions": [{"value": "None", "lang": "en"}], "other": {"anies": [{"name": "referenceToPublisher", "value": {"shortDescription": [{"value": "Institut Bauen und Umwelt e. V.", "lang": "en"}], "type": "contact data set", "refObjectId": "d111dbec-b024-4be5-86c5-752d6eb2cf95", "uri": "../contacts/d111dbec-b024-4be5-86c5-752d6eb2cf95.xml"}}]}}}, "exchanges": {"exchange": [{"dataSetInternalID": 0, "referenceToFlowDataSet": {"shortDescription": [{"value": "PROMATECT®–H (PROMATECT®–H)", "lang": "en"}], "type": "flow data set", "refObjectId": "26645b3d-92a9-7d72-0552-759973674349", "uri": "../flows/26645b3d-92a9-7d72-0552-759973674349.xml"}, "meanAmount": 1.0, "referencesToDataSource": {}, "referenceFlow": true, "resolvedFlowVersion": "00.02.000", "resultingflowAmount": 21.2, "flowProperties": [{"name": [{"lang": "en", "value": "Mass"}, {"lang": "de", "value": "Masse"}], "uuid": "93a60a56-a3c8-11da-a746-0800200b9a66", "referenceFlowProperty": true, "meanValue": 21.2, "referenceUnit": "kg", "unitGroupUUID": "ad38d542-3fe9-439d-9b95-2f5f7752acaf"}], "materialProperties": [{"name": "gross density", "value": "1058.0", "unit": "kg/m^3", "unitDescription": "kilograms per cubic metre"}], "typeOfFlow": "Product flow", "classification": {"classHierarchy": "Dämmstoffe / Calciumsilikat / Calcium-Silikathydrat / Calciumsilikat", "name": "OEKOBAU.DAT"}}, {"dataSetInternalID": 1, "referenceToFlowDataSet": {"shortDescription": [{"value": "Renewable primary energy as energy carrier (PERE)", "lang": "en"}, {"value": "Erneuerbare Primärenergie als Energieträger (PERE)", "lang": "de"}], "type": "flow data set", "refObjectId": "20f32be5-0398-4288-9b6d-accddd195317", "uri": "../flows/20f32be5-0398-4288-9b6d-accddd195317.xml"}, "exchange direction": "INPUT", "other": {"anies": [{"name": "referenceToUnitGroupDataSet", "value": {"shortDescription": [{"value": "MJ", "lang": "en"}], "type": "unit group data set", "refObjectId": "93a60a57-a3c8-11da-a746-0800200c9a66", "uri": "../unitgroups/93a60a57-a3c8-11da-a746-0800200c9a66.xml"}}, {"value": "8.913", "module": "A1"}, {"value": "0.3056", "module": "A2"}, {"value": "9.82", "module": "A3"}, {"value": "0.5797", "module": "A4"}, {"value": "3.672", "module": "A5"}, {"value": "0", "module": "B1", "scenario": "S1"}, {"value": "0", "module": "B1", "scenario": "S2"}, {"value": "0", "module": "B2"}, {"value": "0", "module": "B6"}, {"value": "0", "module": "B7"}, {"value": "0", "module": "C1"}, {"value": "0.1836", "module": "C2", "scenario": "S1"}, {"value": "0.0379", "module": "C2", "scenario": "S2"}, {"value": "0.166", "module": "C3", "scenario": "S1"}, {"value": "0.0004541", "module": "C3", "scenario": "S2"}, {"value": "3.303E-05", "module": "C4", "scenario": "S1"}, {"value": "0.1892", "module": "C4", "scenario": "S2"}, {"value": "0", "module": "D", "scenario": "S1"}, {"value": "0", "module": "D", "scenario": "S2"}]}, "resolvedFlowVersion": "38.00.000", "flowProperties": [], "typeOfFlow": "Other flow", "classification": {"classHierarchy": "Quantities", "name": "GaBiCategories"}}, {"dataSetInternalID": 2, "referenceToFlowDataSet": {"shortDescription": [{"value": "Renewable primary energy resources as material utilization (PERM)", "lang": "en"}, {"value": "Erneuerbare Primärenergie zur stofflichen Nutzung (PERM)", "lang": "de"}], "type": "flow data set", "refObjectId": "fb3ec0de-548d-4508-aea5-00b73bf6f702", "uri": "../flows/fb3ec0de-548d-4508-aea5-00b73bf6f702.xml"}, "exchange direction": "INPUT", "other": {"anies": [{"name": "referenceToUnitGroupDataSet", "value": {"shortDescription": [{"value": "MJ", "lang": "en"}], "type": "unit group data set", "refObjectId": "93a60a57-a3c8-11da-a746-0800200c9a66", "uri": "../unitgroups/93a60a57-a3c8-11da-a746-0800200c9a66.xml"}}, {"value": "9.984", "module": "A1"}, {"value": "0", "module": "A2"}, {"value": "4.729", "module": "A3"}, {"value": "0", "module": "A4"}, {"value": "-2.951", "module": "A5"}, {"value": "0", "module": "B1", "scenario": "S1"}, {"value": "0", "module": "B1", "scenario": "S2"}, {"value": "0", "module": "B2"}, {"value": "0", "module": "B6"}, {"value": "0", "module": "B7"}, {"value": "0", "module": "C1"}, {"value": "0", "module": "C2", "scenario": "S1"}, {"value": "0", "module": "C2", "scenario": "S2"}, {"value": "-9.172", "module": "C3", "scenario": "S1"}, {"value": "0", "module": "C3", "scenario": "S2"}, {"value": "0", "module": "C4", "scenario": "S1"}, {"value": "0", "module": "C4", "scenario": "S2"}, {"value": "11.16", "module": "D", "scenario": "S1"}, {"value": "1.987", "module": "D", "scenario": "S2"}]}, "resolvedFlowVersion": "38.00.000", "flowProperties": [], "typeOfFlow": "Other flow", "classification": {"classHierarchy": "Quantities", "name": "GaBiCategories"}}, {"dataSetInternalID": 3, "referenceToFlowDataSet": {"shortDescription": [{"value": "Total use of renewable primary energy resources (PERT)", "lang": "en"}, {"value": "Total erneuerbare Primärenergie (PERT)", "lang": "de"}], "type": "flow data set", "refObjectId": "53f97275-fa8a-4cdd-9024-65936002acd0", "uri": "../flows/53f97275-fa8a-4cdd-9024-65936002acd0.xml"}, "exchange direction": "INPUT", "other": {"anies": [{"name": "referenceToUnitGroupDataSet", "value": {"shortDescription": [{"value": "MJ", "lang": "en"}], "type": "unit group data set", "refObjectId": "93a60a57-a3c8-11da-a746-0800200c9a66", "uri": "../unitgroups/93a60a57-a3c8-11da-a746-0800200c9a66.xml"}}, {"value": "18.9", "module": "A1"}, {"value": "0.3056", "module": "A2"}, {"value": "14.55", "module": "A3"}, {"value": "0.5797", "module": "A4"}, {"value": "0.7216", "module": "A5"}, {"value": "0", "module": "B1", "scenario": "S1"}, {"value": "0", "module": "B1", "scenario": "S2"}, {"value": "0", "module": "B2"}, {"value": "0", "module": "B6"}, {"value": "0", "module": "B7"}, {"value": "0", "module": "C1"}, {"value": "0.1836", "module": "C2", "scenario": "S1"}, {"value": "0.0379", "module": "C2", "scenario": "S2"}, {"value": "-9.006", "module": "C3", "scenario": "S1"}, {"value": "0.0004541", "module": "C3", "scenario": "S2"}, {"value": "3.303E-05", "module": "C4", "scenario": "S1"}, {"value": "0.1892", "module": "C4", "scenario": "S2"}, {"value": "11.16", "module": "D", "scenario": "S1"}, {"value": "1.987", "module": "D", "scenario": "S2"}]}, "resolvedFlowVersion": "38.00.000", "flowProperties": [], "typeOfFlow": "Other flow", "classification": {"classHierarchy": "Quantities / Environmental quantities / EPD EN 15804 / LCI indicators", "name": "GaBiCategories"}}, {"dataSetInternalID": 4, "referenceToFlowDataSet": {"shortDescription": [{"value": "Non renewable primary energy as energy carrier (PENRE)", "lang": "en"}, {"value": "Nicht-erneuerbare Primärenergie als Energieträger (PENRE)", "lang": "de"}], "type": "flow data set", "refObjectId": "ac857178-2b45-46ec-892a-a9a4332f0372", "uri": "../flows/ac857178-2b45-46ec-892a-a9a4332f0372.xml"}, "exchange direction": "INPUT", "other": {"anies": [{"name": "referenceToUnitGroupDataSet", "value": {"shortDescription": [{"value": "MJ", "lang": "en"}], "type": "unit group data set", "refObjectId": "93a60a57-a3c8-11da-a746-0800200c9a66", "uri": "../unitgroups/93a60a57-a3c8-11da-a746-0800200c9a66.xml"}}, {"value": "40.64", "module": "A1"}, {"value": "20.48", "module": "A2"}, {"value": "135.8", "module": "A3"}, {"value": "62.92", "module": "A4"}, {"value": "22.67", "module": "A5"}, {"value": "0", "module": "B1", "scenario": "S1"}, {"value": "0", "module": "B1", "scenario": "S2"}, {"value": "0", "module": "B2"}, {"value": "0", "module": "B6"}, {"value": "0", "module": "B7"}, {"value": "0", "module": "C1"}, {"value": "13.13", "module": "C2", "scenario": "S1"}, {"value": "2.711", "module": "C2", "scenario": "S2"}, {"value": "1.217", "module": "C3", "scenario": "S1"}, {"value": "0.002745", "module": "C3", "scenario": "S2"}, {"value": "0.0008027", "module": "C4", "scenario": "S1"}, {"value": "3.761", "module": "C4", "scenario": "S2"}, {"value": "0", "module": "D", "scenario": "S1"}, {"value": "0", "module": "D", "scenario": "S2"}]}, "resolvedFlowVersion": "38.00.000", "flowProperties": [], "typeOfFlow": "Other flow", "classification": {"classHierarchy": "Quantities", "name": "GaBiCategories"}}, {"dataSetInternalID": 5, "referenceToFlowDataSet": {"shortDescription": [{"value": "Non renewable primary energy as material utilization (PENRM)", "lang": "en"}, {"value": "Nicht-erneuerbare Primärenergie zur stofflichen Nutzung (PENRM)", "lang": "de"}], "type": "flow data set", "refObjectId": "1421caa0-679d-4bf4-b282-0eb850ccae27", "uri": "../flows/1421caa0-679d-4bf4-b282-0eb850ccae27.xml"}, "exchange direction": "INPUT", "other": {"anies": [{"name": "referenceToUnitGroupDataSet", "value": {"shortDescription": [{"value": "MJ", "lang": "en"}], "type": "unit group data set", "refObjectId": "93a60a57-a3c8-11da-a746-0800200c9a66", "uri": "../unitgroups/93a60a57-a3c8-11da-a746-0800200c9a66.xml"}}, {"value": "0.2341", "module": "A1"}, {"value": "0", "module": "A2"}, {"value": "0.1502", "module": "A3"}, {"value": "0", "module": "A4"}, {"value": "-0.1623", "module": "A5"}, {"value": "0", "module": "B1", "scenario": "S1"}, {"value": "0", "module": "B1", "scenario": "S2"}, {"value": "0", "module": "B2"}, {"value": "0", "module": "B6"}, {"value": "0", "module": "B7"}, {"value": "0", "module": "C1"}, {"value": "0", "module": "C2", "scenario": "S1"}, {"value": "0", "module": "C2", "scenario": "S2"}, {"value": "0", "module": "C3", "scenario": "S1"}, {"value": "0", "module": "C3", "scenario": "S2"}, {"value": "0", "module": "C4", "scenario": "S1"}, {"value": "0", "module": "C4", "scenario": "S2"}, {"value": "0.1609", "module": "D", "scenario": "S1"}, {"value": "0.1609", "module": "D", "scenario": "S2"}]}, "resolvedFlowVersion": "38.00.000", "flowProperties": [], "typeOfFlow": "Other flow", "classification": {"classHierarchy": "Quantities", "name": "GaBiCategories"}}, {"dataSetInternalID": 6, "referenceToFlowDataSet": {"shortDescription": [{"value": "Total use of non renewable primary energy resources (PENRT)", "lang": "en"}, {"value": "Total nicht erneuerbare Primärenergie (PENRT)", "lang": "de"}], "type": "flow data set", "refObjectId": "06159210-646b-4c8d-8583-da9b3b95a6c1", "uri": "../flows/06159210-646b-4c8d-8583-da9b3b95a6c1.xml"}, "exchange direction": "INPUT", "other": {"anies": [{"name": "referenceToUnitGroupDataSet", "value": {"shortDescription": [{"value": "MJ", "lang": "en"}], "type": "unit group data set", "refObjectId": "93a60a57-a3c8-11da-a746-0800200c9a66", "uri": "../unitgroups/93a60a57-a3c8-11da-a746-0800200c9a66.xml"}}, {"value": "40.87", "module": "A1"}, {"value": "20.48", "module": "A2"}, {"value": "135.9", "module": "A3"}, {"value": "62.92", "module": "A4"}, {"value": "22.51", "module": "A5"}, {"value": "0", "module": "B1", "scenario": "S1"}, {"value": "0", "module": "B1", "scenario": "S2"}, {"value": "0", "module": "B2"}, {"value": "0", "module": "B6"}, {"value": "0", "module": "B7"}, {"value": "0", "module": "C1"}, {"value": "13.13", "module": "C2", "scenario": "S1"}, {"value": "2.711", "module": "C2", "scenario": "S2"}, {"value": "1.217", "module": "C3", "scenario": "S1"}, {"value": "0.002745", "module": "C3", "scenario": "S2"}, {"value": "0.0008027", "module": "C4", "scenario": "S1"}, {"value": "3.761", "module": "C4", "scenario": "S2"}, {"value": "0.1609", "module": "D", "scenario": "S1"}, {"value": "0.1609", "module": "D", "scenario": "S2"}]}, "resolvedFlowVersion": "38.00.000", "flowProperties": [], "typeOfFlow": "Other flow", "classification": {"classHierarchy": "Quantities / Environmental quantities / EPD EN 15804 / LCI indicators", "name": "GaBiCategories"}}, {"dataSetInternalID": 7, "referenceToFlowDataSet": {"shortDescription": [{"value": "Use of secondary material (SM)", "lang": "en"}, {"value": "Einsatz von Sekundärstoffen (SM)", "lang": "de"}], "type": "flow data set", "refObjectId": "c6a1f35f-2d09-4f54-8dfb-97e502e1ce92", "uri": "../flows/c6a1f35f-2d09-4f54-8dfb-97e502e1ce92.xml"}, "exchange direction": "INPUT", "other": {"anies": [{"name": "referenceToUnitGroupDataSet", "value": {"shortDescription": [{"value": "kg", "lang": "en"}], "type": "unit group data set", "refObjectId": "ad38d542-3fe9-439d-9b95-2f5f7752acaf", "uri": "../unitgroups/ad38d542-3fe9-439d-9b95-2f5f7752acaf.xml"}}, {"value": "0", "module": "A1"}, {"value": "0", "module": "A2"}, {"value": "0", "module": "A3"}, {"value": "0", "module": "A4"}, {"value": "0", "module": "A5"}, {"value": "0", "module": "B1", "scenario": "S1"}, {"value": "0", "module": "B1", "scenario": "S2"}, {"value": "0", "module": "B2"}, {"value": "0", "module": "B6"}, {"value": "0", "module": "B7"}, {"value": "0", "module": "C1"}, {"value": "0", "module": "C2", "scenario": "S1"}, {"value": "0", "module": "C2", "scenario": "S2"}, {"value": "0", "module": "C3", "scenario": "S1"}, {"value": "0", "module": "C3", "scenario": "S2"}, {"value": "0", "module": "C4", "scenario": "S1"}, {"value": "0", "module": "C4", "scenario": "S2"}, {"value": "0", "module": "D", "scenario": "S1"}, {"value": "0", "module": "D", "scenario": "S2"}]}, "resolvedFlowVersion": "38.00.000", "flowProperties": [], "typeOfFlow": "Other flow", "classification": {"classHierarchy": "Quantities / Environmental quantities / EPD EN 15804 / LCI indicators", "name": "GaBiCategories"}}, {"dataSetInternalID": 8, "referenceToFlowDataSet": {"shortDescription": [{"value": "Use of renewable secondary fuels (RSF)", "lang": "en"}, {"value": "Erneuerbare Sekundärbrennstoffe (RSF)", "lang": "de"}], "type": "flow data set", "refObjectId": "64333088-a55f-4aa2-9a31-c10b07816787", "uri": "../flows/64333088-a55f-4aa2-9a31-c10b07816787.xml"}, "exchange direction": "INPUT", "other": {"anies": [{"name": "referenceToUnitGroupDataSet", "value": {"shortDescription": [{"value": "MJ", "lang": "en"}], "type": "unit group data set", "refObjectId": "93a60a57-a3c8-11da-a746-0800200c9a66", "uri": "../unitgroups/93a60a57-a3c8-11da-a746-0800200c9a66.xml"}}, {"value": "0", "module": "A1"}, {"value": "0", "module": "A2"}, {"value": "0", "module": "A3"}, {"value": "0", "module": "A4"}, {"value": "0", "module": "A5"}, {"value": "0", "module": "B1", "scenario": "S1"}, {"value": "0", "module": "B1", "scenario": "S2"}, {"value": "0", "module": "B2"}, {"value": "0", "module": "B6"}, {"value": "0", "module": "B7"}, {"value": "0", "module": "C1"}, {"value": "0", "module": "C2", "scenario": "S1"}, {"value": "0", "module": "C2", "scenario": "S2"}, {"value": "0", "module": "C3", "scenario": "S1"}, {"value": "0", "module": "C3", "scenario": "S2"}, {"value": "0", "module": "C4", "scenario": "S1"}, {"value": "0", "module": "C4", "scenario": "S2"}, {"value": "0", "module": "D", "scenario": "S1"}, {"value": "0", "module": "D", "scenario": "S2"}]}, "resolvedFlowVersion": "38.00.000", "flowProperties": [], "typeOfFlow": "Other flow", "classification": {"classHierarchy": "Quantities / Environmental quantities / EPD EN 15804 / LCI indicators", "name": "GaBiCategories"}}, {"dataSetInternalID": 9, "referenceToFlowDataSet": {"shortDescription": [{"value": "Use of non renewable secondary fuels (NRSF)", "lang": "en"}, {"value": "Nicht erneuerbare Sekundärbrennstoffe (NRSF)", "lang": "de"}], "type": "flow data set", "refObjectId": "89def144-d39a-4287-b86f-efde453ddcb2", "uri": "../flows/89def144-d39a-4287-b86f-efde453ddcb2.xml"}, "exchange direction": "INPUT", "other": {"anies": [{"name": "referenceToUnitGroupDataSet", "value": {"shortDescription": [{"value": "MJ", "lang": "en"}], "type": "unit group data set", "refObjectId": "93a60a57-a3c8-11da-a746-0800200c9a66", "uri": "../unitgroups/93a60a57-a3c8-11da-a746-0800200c9a66.xml"}}, {"value": "0", "module": "A1"}, {"value": "0", "module": "A2"}, {"value": "0", "module": "A3"}, {"value": "0", "module": "A4"}, {"value": "0", "module": "A5"}, {"value": "0", "module": "B1", "scenario": "S1"}, {"value": "0", "module": "B1", "scenario": "S2"}, {"value": "0", "module": "B2"}, {"value": "0", "module": "B6"}, {"value": "0", "module": "B7"}, {"value": "0", "module": "C1"}, {"value": "0", "module": "C2", "scenario": "S1"}, {"value": "0", "module": "C2", "scenario": "S2"}, {"value": "0", "module": "C3", "scenario": "S1"}, {"value": "0", "module": "C3", "scenario": "S2"}, {"value": "0", "module": "C4", "scenario": "S1"}, {"value": "0", "module": "C4", "scenario": "S2"}, {"value": "0", "module": "D", "scenario": "S1"}, {"value": "0", "module": "D", "scenario": "S2"}]}, "resolvedFlowVersion": "38.00.000", "flowProperties": [], "typeOfFlow": "Other flow", "classification": {"classHierarchy": "Quantities / Environmental quantities / EPD EN 15804 / LCI indicators", "name": "GaBiCategories"}}, {"dataSetInternalID": 10, "referenceToFlowDataSet": {"shortDescription": [{"value": "Use of net fresh water (FW)", "lang": "en"}, {"value": "Einsatz von Süßwasserressourcen (FW)", "lang": "de"}], "type": "flow data set", "refObjectId": "3cf952c8-f3a4-461d-8c96-96456ca62246", "uri": "../flows/3cf952c8-f3a4-461d-8c96-96456ca62246.xml"}, "exchange direction": "INPUT", "other": {"anies": [{"name": "referenceToUnitGroupDataSet", "value": {"shortDescription": [{"value": "m^3", "lang": "en"}], "type": "unit group data set", "refObjectId": "cd950537-0a98-4044-9ba7-9f9a68d0a504", "uri": "../unitgroups/cd950537-0a98-4044-9ba7-9f9a68d0a504.xml"}}, {"value": "0.02348", "module": "A1"}, {"value": "0.001329", "module": "A2"}, {"value": "0.01363", "module": "A3"}, {"value": "0.002928", "module": "A4"}, {"value": "0.006474", "module": "A5"}, {"value": "0", "module": "B1", "scenario": "S1"}, {"value": "0", "module": "B1", "scenario": "S2"}, {"value": "0", "module": "B2"}, {"value": "0", "module": "B6"}, {"value": "0", "module": "B7"}, {"value": "0", "module": "C1"}, {"value": "0.0009604", "module": "C2", "scenario": "S1"}, {"value": "0.0001983", "module": "C2", "scenario": "S2"}, {"value": "0.001049", "module": "C3", "scenario": "S1"}, {"value": "1.725E-06", "module": "C3", "scenario": "S2"}, {"value": "-1.144E-07", "module": "C4", "scenario": "S1"}, {"value": "0.003939", "module": "C4", "scenario": "S2"}, {"value": "-0.03242", "module": "D", "scenario": "S1"}, {"value": "-0.001675", "module": "D", "scenario": "S2"}]}, "resolvedFlowVersion": "38.00.000", "flowProperties": [], "typeOfFlow": "Other flow", "classification": {"classHierarchy": "Quantities / Environmental quantities / EPD EN 15804 / LCI indicators", "name": "GaBiCategories"}}, {"dataSetInternalID": 11, "referenceToFlowDataSet": {"shortDescription": [{"value": "Hazardous waste disposed (HWD)", "lang": "en"}, {"value": "Gefährlicher Abfall zur Deponie (HWD)", "lang": "de"}], "type": "flow data set", "refObjectId": "430f9e0f-59b2-46a0-8e0d-55e0e84948fc", "uri": "../flows/430f9e0f-59b2-46a0-8e0d-55e0e84948fc.xml"}, "exchange direction": "OUTPUT", "other": {"anies": [{"name": "referenceToUnitGroupDataSet", "value": {"shortDescription": [{"value": "kg", "lang": "en"}], "type": "unit group data set", "refObjectId": "ad38d542-3fe9-439d-9b95-2f5f7752acaf", "uri": "../unitgroups/ad38d542-3fe9-439d-9b95-2f5f7752acaf.xml"}}, {"value": "3.313E-05", "module": "A1"}, {"value": "5.056E-05", "module": "A2"}, {"value": "0.000114", "module": "A3"}, {"value": "9.636E-05", "module": "A4"}, {"value": "2.305E-05", "module": "A5"}, {"value": "0", "module": "B1", "scenario": "S1"}, {"value": "0", "module": "B1", "scenario": "S2"}, {"value": "0", "module": "B2"}, {"value": "0", "module": "B6"}, {"value": "0", "module": "B7"}, {"value": "0", "module": "C1"}, {"value": "3.409E-05", "module": "C2", "scenario": "S1"}, {"value": "7.038E-06", "module": "C2", "scenario": "S2"}, {"value": "1.211E-06", "module": "C3", "scenario": "S1"}, {"value": "1.894E-09", "module": "C3", "scenario": "S2"}, {"value": "1.314E-09", "module": "C4", "scenario": "S1"}, {"value": "4.016E-06", "module": "C4", "scenario": "S2"}, {"value": "-1.475E-05", "module": "D", "scenario": "S1"}, {"value": "-8.218E-06", "module": "D", "scenario": "S2"}]}, "resolvedFlowVersion": "38.00.000", "flowProperties": [], "typeOfFlow": "Other flow", "classification": {"classHierarchy": "Quantities / Environmental quantities / EPD EN 15804 / LCI indicators", "name": "GaBiCategories"}}, {"dataSetInternalID": 12, "referenceToFlowDataSet": {"shortDescription": [{"value": "Non hazardous waste disposed (NHWD)", "lang": "en"}, {"value": "Entsorgter nicht gefährlicher Abfall (NHWD)", "lang": "de"}], "type": "flow data set", "refObjectId": "b29ef66b-e286-4afa-949f-62f1a7b4d7fa", "uri": "../flows/b29ef66b-e286-4afa-949f-62f1a7b4d7fa.xml"}, "exchange direction": "OUTPUT", "other": {"anies": [{"name": "referenceToUnitGroupDataSet", "value": {"shortDescription": [{"value": "kg", "lang": "en"}], "type": "unit group data set", "refObjectId": "ad38d542-3fe9-439d-9b95-2f5f7752acaf", "uri": "../unitgroups/ad38d542-3fe9-439d-9b95-2f5f7752acaf.xml"}}, {"value": "0.2275", "module": "A1"}, {"value": "0.6308", "module": "A2"}, {"value": "0.5996", "module": "A3"}, {"value": "1.274", "module": "A4"}, {"value": "0.7988", "module": "A5"}, {"value": "0", "module": "B1", "scenario": "S1"}, {"value": "0", "module": "B1", "scenario": "S2"}, {"value": "0", "module": "B2"}, {"value": "0", "module": "B6"}, {"value": "0", "module": "B7"}, {"value": "0", "module": "C1"}, {"value": "0.6841", "module": "C2", "scenario": "S1"}, {"value": "0.1412", "module": "C2", "scenario": "S2"}, {"value": "0.01526", "module": "C3", "scenario": "S1"}, {"value": "8.993E-06", "module": "C3", "scenario": "S2"}, {"value": "0.003088", "module": "C4", "scenario": "S1"}, {"value": "21.14", "module": "C4", "scenario": "S2"}, {"value": "-0.01809", "module": "D", "scenario": "S1"}, {"value": "-0.003075", "module": "D", "scenario": "S2"}]}, "resolvedFlowVersion": "38.00.000", "flowProperties": [], "typeOfFlow": "Other flow", "classification": {"classHierarchy": "Quantities / Environmental quantities / EPD EN 15804 / LCI indicators", "name": "GaBiCategories"}}, {"dataSetInternalID": 13, "referenceToFlowDataSet": {"shortDescription": [{"value": "Radioactive waste disposed (RWD)", "lang": "en"}, {"value": "Entsorgter radioaktiver Abfall (RWD)", "lang": "de"}], "type": "flow data set", "refObjectId": "3449546e-52ad-4b39-b809-9fb77cea8ff6", "uri": "../flows/3449546e-52ad-4b39-b809-9fb77cea8ff6.xml"}, "exchange direction": "OUTPUT", "other": {"anies": [{"name": "referenceToUnitGroupDataSet", "value": {"shortDescription": [{"value": "kg", "lang": "en"}], "type": "unit group data set", "refObjectId": "ad38d542-3fe9-439d-9b95-2f5f7752acaf", "uri": "../unitgroups/ad38d542-3fe9-439d-9b95-2f5f7752acaf.xml"}}, {"value": "0.0001632", "module": "A1"}, {"value": "0.0001291", "module": "A2"}, {"value": "0.000157", "module": "A3"}, {"value": "0.0004328", "module": "A4"}, {"value": "7.248E-05", "module": "A5"}, {"value": "0", "module": "B1", "scenario": "S1"}, {"value": "0", "module": "B1", "scenario": "S2"}, {"value": "0", "module": "B2"}, {"value": "0", "module": "B6"}, {"value": "0", "module": "B7"}, {"value": "0", "module": "C1"}, {"value": "8.824E-05", "module": "C2", "scenario": "S1"}, {"value": "1.822E-05", "module": "C2", "scenario": "S2"}, {"value": "6.871E-06", "module": "C3", "scenario": "S1"}, {"value": "1.678E-08", "module": "C3", "scenario": "S2"}, {"value": "4.723E-09", "module": "C4", "scenario": "S1"}, {"value": "2.504E-05", "module": "C4", "scenario": "S2"}, {"value": "-2.755E-05", "module": "D", "scenario": "S1"}, {"value": "-4.796E-06", "module": "D", "scenario": "S2"}]}, "resolvedFlowVersion": "38.00.000", "flowProperties": [], "typeOfFlow": "Other flow", "classification": {"classHierarchy": "Quantities / Environmental quantities / EPD EN 15804 / LCI indicators", "name": "GaBiCategories"}}, {"dataSetInternalID": 14, "referenceToFlowDataSet": {"shortDescription": [{"value": "Components for re-use (CRU)", "lang": "en"}, {"value": "Komponenten für die Wiederverwendung (CRU)", "lang": "de"}], "type": "flow data set", "refObjectId": "a2b32f97-3fc7-4af2-b209-525bc6426f33", "uri": "../flows/a2b32f97-3fc7-4af2-b209-525bc6426f33.xml"}, "exchange direction": "OUTPUT", "other": {"anies": [{"name": "referenceToUnitGroupDataSet", "value": {"shortDescription": [{"value": "kg", "lang": "en"}], "type": "unit group data set", "refObjectId": "ad38d542-3fe9-439d-9b95-2f5f7752acaf", "uri": "../unitgroups/ad38d542-3fe9-439d-9b95-2f5f7752acaf.xml"}}, {"value": "0", "module": "A1"}, {"value": "0", "module": "A2"}, {"value": "0", "module": "A3"}, {"value": "0", "module": "A4"}, {"value": "0", "module": "A5"}, {"value": "0", "module": "B1", "scenario": "S1"}, {"value": "0", "module": "B1", "scenario": "S2"}, {"value": "0", "module": "B2"}, {"value": "0", "module": "B6"}, {"value": "0", "module": "B7"}, {"value": "0", "module": "C1"}, {"value": "0", "module": "C2", "scenario": "S1"}, {"value": "0", "module": "C2", "scenario": "S2"}, {"value": "0", "module": "C3", "scenario": "S1"}, {"value": "0", "module": "C3", "scenario": "S2"}, {"value": "0", "module": "C4", "scenario": "S1"}, {"value": "0", "module": "C4", "scenario": "S2"}, {"value": "0", "module": "D", "scenario": "S1"}, {"value": "0", "module": "D", "scenario": "S2"}]}, "resolvedFlowVersion": "38.00.000", "flowProperties": [], "typeOfFlow": "Other flow", "classification": {"classHierarchy": "Quantities / Environmental quantities / EPD EN 15804 / LCI indicators", "name": "GaBiCategories"}}, {"dataSetInternalID": 15, "referenceToFlowDataSet": {"shortDescription": [{"value": "Materials for recycling (MFR)", "lang": "en"}, {"value": "Stoffe zum Recycling (MFR)", "lang": "de"}], "type": "flow data set", "refObjectId": "d7fe48a5-4103-49c8-9aae-b0b5dfdbd6ae", "uri": "../flows/d7fe48a5-4103-49c8-9aae-b0b5dfdbd6ae.xml"}, "exchange direction": "OUTPUT", "other": {"anies": [{"name": "referenceToUnitGroupDataSet", "value": {"shortDescription": [{"value": "kg", "lang": "en"}], "type": "unit group data set", "refObjectId": "ad38d542-3fe9-439d-9b95-2f5f7752acaf", "uri": "../unitgroups/ad38d542-3fe9-439d-9b95-2f5f7752acaf.xml"}}, {"value": "0", "module": "A1"}, {"value": "0", "module": "A2"}, {"value": "0.004789", "module": "A3"}, {"value": "0", "module": "A4"}, {"value": "1.221", "module": "A5"}, {"value": "0", "module": "B1", "scenario": "S1"}, {"value": "0", "module": "B1", "scenario": "S2"}, {"value": "0", "module": "B2"}, {"value": "0", "module": "B6"}, {"value": "0", "module": "B7"}, {"value": "0", "module": "C1"}, {"value": "0", "module": "C2", "scenario": "S1"}, {"value": "0", "module": "C2", "scenario": "S2"}, {"value": "21.22", "module": "C3", "scenario": "S1"}, {"value": "0.07324", "module": "C3", "scenario": "S2"}, {"value": "0", "module": "C4", "scenario": "S1"}, {"value": "0", "module": "C4", "scenario": "S2"}, {"value": "0", "module": "D", "scenario": "S1"}, {"value": "0", "module": "D", "scenario": "S2"}]}, "resolvedFlowVersion": "38.00.000", "flowProperties": [], "typeOfFlow": "Other flow", "classification": {"classHierarchy": "Quantities / Environmental quantities / EPD EN 15804 / LCI indicators", "name": "GaBiCategories"}}, {"dataSetInternalID": 16, "referenceToFlowDataSet": {"shortDescription": [{"value": "Materials for energy recovery (MER)", "lang": "en"}, {"value": "Stoffe für die Energierückgewinnung (MER)", "lang": "de"}], "type": "flow data set", "refObjectId": "59a9181c-3aaf-46ee-8b13-2b3723b6e447", "uri": "../flows/59a9181c-3aaf-46ee-8b13-2b3723b6e447.xml"}, "exchange direction": "OUTPUT", "other": {"anies": [{"name": "referenceToUnitGroupDataSet", "value": {"shortDescription": [{"value": "kg", "lang": "en"}], "type": "unit group data set", "refObjectId": "ad38d542-3fe9-439d-9b95-2f5f7752acaf", "uri": "../unitgroups/ad38d542-3fe9-439d-9b95-2f5f7752acaf.xml"}}, {"value": "0", "module": "A1"}, {"value": "0", "module": "A2"}, {"value": "0", "module": "A3"}, {"value": "0", "module": "A4"}, {"value": "0", "module": "A5"}, {"value": "0", "module": "B1", "scenario": "S1"}, {"value": "0", "module": "B1", "scenario": "S2"}, {"value": "0", "module": "B2"}, {"value": "0", "module": "B6"}, {"value": "0", "module": "B7"}, {"value": "0", "module": "C1"}, {"value": "0", "module": "C2", "scenario": "S1"}, {"value": "0", "module": "C2", "scenario": "S2"}, {"value": "0", "module": "C3", "scenario": "S1"}, {"value": "0", "module": "C3", "scenario": "S2"}, {"value": "0", "module": "C4", "scenario": "S1"}, {"value": "0", "module": "C4", "scenario": "S2"}, {"value": "0", "module": "D", "scenario": "S1"}, {"value": "0", "module": "D", "scenario": "S2"}]}, "resolvedFlowVersion": "38.00.000", "flowProperties": [], "typeOfFlow": "Other flow", "classification": {"classHierarchy": "Quantities / Environmental quantities / EPD EN 15804 / LCI indicators", "name": "GaBiCategories"}}, {"dataSetInternalID": 17, "referenceToFlowDataSet": {"shortDescription": [{"value": "Exported electrical energy (EEE)", "lang": "en"}, {"value": "Exportierte elektrische Energie (EEE)", "lang": "de"}], "type": "flow data set", "refObjectId": "4da0c987-2b76-40d6-9e9e-82a017aaaf29", "uri": "../flows/4da0c987-2b76-40d6-9e9e-82a017aaaf29.xml"}, "exchange direction": "OUTPUT", "other": {"anies": [{"name": "referenceToUnitGroupDataSet", "value": {"shortDescription": [{"value": "MJ", "lang": "en"}], "type": "unit group data set", "refObjectId": "93a60a57-a3c8-11da-a746-0800200c9a66", "uri": "../unitgroups/93a60a57-a3c8-11da-a746-0800200c9a66.xml"}}, {"value": "0", "module": "A1"}, {"value": "0", "module": "A2"}, {"value": "0.0072", "module": "A3"}, {"value": "0", "module": "A4"}, {"value": "0.134", "module": "A5"}, {"value": "0", "module": "B1", "scenario": "S1"}, {"value": "0", "module": "B1", "scenario": "S2"}, {"value": "0", "module": "B2"}, {"value": "0", "module": "B6"}, {"value": "0", "module": "B7"}, {"value": "0", "module": "C1"}, {"value": "0", "module": "C2", "scenario": "S1"}, {"value": "0", "module": "C2", "scenario": "S2"}, {"value": "0", "module": "C3", "scenario": "S1"}, {"value": "0", "module": "C3", "scenario": "S2"}, {"value": "0", "module": "C4", "scenario": "S1"}, {"value": "0", "module": "C4", "scenario": "S2"}, {"value": "0", "module": "D", "scenario": "S1"}, {"value": "0", "module": "D", "scenario": "S2"}]}, "resolvedFlowVersion": "38.00.000", "flowProperties": [], "typeOfFlow": "Other flow", "classification": {"classHierarchy": "Quantities / Environmental quantities / EPD EN 15804 / LCI indicators", "name": "GaBiCategories"}}, {"dataSetInternalID": 18, "referenceToFlowDataSet": {"shortDescription": [{"value": "Exported thermal energy (EET)", "lang": "en"}, {"value": "Exportierte thermische Energie (EET)", "lang": "de"}], "type": "flow data set", "refObjectId": "98daf38a-7a79-46d3-9a37-2b7bd0955810", "uri": "../flows/98daf38a-7a79-46d3-9a37-2b7bd0955810.xml"}, "exchange direction": "OUTPUT", "other": {"anies": [{"name": "referenceToUnitGroupDataSet", "value": {"shortDescription": [{"value": "MJ", "lang": "en"}], "type": "unit group data set", "refObjectId": "93a60a57-a3c8-11da-a746-0800200c9a66", "uri": "../unitgroups/93a60a57-a3c8-11da-a746-0800200c9a66.xml"}}, {"value": "0", "module": "A1"}, {"value": "0", "module": "A2"}, {"value": "0.0144", "module": "A3"}, {"value": "0", "module": "A4"}, {"value": "0.2681", "module": "A5"}, {"value": "0", "module": "B1", "scenario": "S1"}, {"value": "0", "module": "B1", "scenario": "S2"}, {"value": "0", "module": "B2"}, {"value": "0", "module": "B6"}, {"value": "0", "module": "B7"}, {"value": "0", "module": "C1"}, {"value": "0", "module": "C2", "scenario": "S1"}, {"value": "0", "module": "C2", "scenario": "S2"}, {"value": "0", "module": "C3", "scenario": "S1"}, {"value": "0", "module": "C3", "scenario": "S2"}, {"value": "0", "module": "C4", "scenario": "S1"}, {"value": "0", "module": "C4", "scenario": "S2"}, {"value": "0", "module": "D", "scenario": "S1"}, {"value": "0", "module": "D", "scenario": "S2"}]}, "resolvedFlowVersion": "38.00.000", "flowProperties": [], "typeOfFlow": "Other flow", "classification": {"classHierarchy": "Quantities / Environmental quantities / EPD EN 15804 / LCI indicators", "name": "GaBiCategories"}}]}, "LCIAResults": {"LCIAResult": [{"referenceToLCIAMethodDataSet": {"shortDescription": [{"value": "Global Warming Potential total (GWP-total)", "lang": "en"}, {"value": "Globales Erwärmungspotenzial total (GWP-total)", "lang": "de"}], "type": "LCIA method data set", "refObjectId": "6a37f984-a4b3-458a-a20a-64418c145fa2", "uri": "../lciamethods/6a37f984-a4b3-458a-a20a-64418c145fa2.xml"}, "other": {"anies": [{"name": "referenceToUnitGroupDataSet", "value": {"shortDescription": [{"value": "kg CO_(2) eq", "lang": "en"}], "type": "unit group data set", "refObjectId": "1ebf3012-d0db-4de2-aefd-ef30cedb0be1", "uri": "../unitgroups/1ebf3012-d0db-4de2-aefd-ef30cedb0be1.xml"}}, {"value": "5.837", "module": "A1"}, {"value": "1.454", "module": "A2"}, {"value": "9.166", "module": "A3"}, {"value": "4.655", "module": "A4"}, {"value": "2.253", "module": "A5"}, {"value": "-2.67", "module": "B1", "scenario": "S1"}, {"value": "-1.42", "module": "B1", "scenario": "S2"}, {"value": "0", "module": "B2"}, {"value": "0", "module": "B6"}, {"value": "0", "module": "B7"}, {"value": "0", "module": "C1"}, {"value": "0.8621", "module": "C2", "scenario": "S1"}, {"value": "0.178", "module": "C2", "scenario": "S2"}, {"value": "1.111", "module": "C3", "scenario": "S1"}, {"value": "0.0001113", "module": "C3", "scenario": "S2"}, {"value": "3.578E-05", "module": "C4", "scenario": "S1"}, {"value": "1.18", "module": "C4", "scenario": "S2"}, {"value": "-0.5993", "module": "D", "scenario": "S1"}, {"value": "-0.3232", "module": "D", "scenario": "S2"}]}}, {"referenceToLCIAMethodDataSet": {"shortDescription": [{"value": "Global Warming Potential fossil fuels (GWP-fossil)", "lang": "en"}, {"value": "Globales Erwärmungspotenzial fossil (GWP-fossil)", "lang": "de"}], "type": "LCIA method data set", "refObjectId": "5f635281-343e-44fb-83df-1971b155e6b6", "uri": "../lciamethods/5f635281-343e-44fb-83df-1971b155e6b6.xml"}, "other": {"anies": [{"name": "referenceToUnitGroupDataSet", "value": {"shortDescription": [{"value": "kg CO_(2) eq", "lang": "en"}], "type": "unit group data set", "refObjectId": "1ebf3012-d0db-4de2-aefd-ef30cedb0be1", "uri": "../unitgroups/1ebf3012-d0db-4de2-aefd-ef30cedb0be1.xml"}}, {"value": "6.918", "module": "A1"}, {"value": "1.451", "module": "A2"}, {"value": "9.646", "module": "A3"}, {"value": "4.651", "module": "A4"}, {"value": "1.767", "module": "A5"}, {"value": "-2.67", "module": "B1", "scenario": "S1"}, {"value": "-1.42", "module": "B1", "scenario": "S2"}, {"value": "0", "module": "B2"}, {"value": "0", "module": "B6"}, {"value": "0", "module": "B7"}, {"value": "0", "module": "C1"}, {"value": "0.8614", "module": "C2", "scenario": "S1"}, {"value": "0.1778", "module": "C2", "scenario": "S2"}, {"value": "0.05948", "module": "C3", "scenario": "S1"}, {"value": "0.0001104", "module": "C3", "scenario": "S2"}, {"value": "3.552E-05", "module": "C4", "scenario": "S1"}, {"value": "0.1283", "module": "C4", "scenario": "S2"}, {"value": "-0.3946", "module": "D", "scenario": "S1"}, {"value": "-0.1197", "module": "D", "scenario": "S2"}]}}, {"referenceToLCIAMethodDataSet": {"shortDescription": [{"value": "Global Warming Potential biogenic (GWP-biogenic)", "lang": "en"}, {"value": "Globales Erwärmungspotenzial biogen (GWP-biogenic)", "lang": "de"}], "type": "LCIA method data set", "refObjectId": "2356e1ab-0185-4db5-86e5-16de51c7485c", "uri": "../lciamethods/2356e1ab-0185-4db5-86e5-16de51c7485c.xml"}, "other": {"anies": [{"name": "referenceToUnitGroupDataSet", "value": {"shortDescription": [{"value": "kg CO_(2) eq", "lang": "en"}], "type": "unit group data set", "refObjectId": "1ebf3012-d0db-4de2-aefd-ef30cedb0be1", "uri": "../unitgroups/1ebf3012-d0db-4de2-aefd-ef30cedb0be1.xml"}}, {"value": "-1.091", "module": "A1"}, {"value": "0.0006805", "module": "A2"}, {"value": "-0.4837", "module": "A3"}, {"value": "0.001253", "module": "A4"}, {"value": "0.4825", "module": "A5"}, {"value": "0", "module": "B1", "scenario": "S1"}, {"value": "0", "module": "B1", "scenario": "S2"}, {"value": "0", "module": "B2"}, {"value": "0", "module": "B6"}, {"value": "0", "module": "B7"}, {"value": "0", "module": "C1"}, {"value": "0.0003081", "module": "C2", "scenario": "S1"}, {"value": "6.362E-05", "module": "C2", "scenario": "S2"}, {"value": "1.051", "module": "C3", "scenario": "S1"}, {"value": "5.977E-07", "module": "C3", "scenario": "S2"}, {"value": "7.852E-08", "module": "C4", "scenario": "S1"}, {"value": "1.051", "module": "C4", "scenario": "S2"}, {"value": "-0.204", "module": "D", "scenario": "S1"}, {"value": "-0.2032", "module": "D", "scenario": "S2"}]}}, {"referenceToLCIAMethodDataSet": {"shortDescription": [{"value": "Global Warming Potential luluc (GWP-luluc)", "lang": "en"}, {"value": "Globales Erwärmungspotenzial luluc (GWP-luluc)", "lang": "de"}], "type": "LCIA method data set", "refObjectId": "4331bbdb-978a-490d-8707-eeb047f01a55", "uri": "../lciamethods/4331bbdb-978a-490d-8707-eeb047f01a55.xml"}, "other": {"anies": [{"name": "referenceToUnitGroupDataSet", "value": {"shortDescription": [{"value": "kg CO_(2) eq", "lang": "en"}], "type": "unit group data set", "refObjectId": "1ebf3012-d0db-4de2-aefd-ef30cedb0be1", "uri": "../unitgroups/1ebf3012-d0db-4de2-aefd-ef30cedb0be1.xml"}}, {"value": "0.003648", "module": "A1"}, {"value": "0.001634", "module": "A2"}, {"value": "0.002276", "module": "A3"}, {"value": "0.002906", "module": "A4"}, {"value": "0.001146", "module": "A5"}, {"value": "0", "module": "B1", "scenario": "S1"}, {"value": "0", "module": "B1", "scenario": "S2"}, {"value": "0", "module": "B2"}, {"value": "0", "module": "B6"}, {"value": "0", "module": "B7"}, {"value": "0", "module": "C1"}, {"value": "0.0003445", "module": "C2", "scenario": "S1"}, {"value": "7.112E-05", "module": "C2", "scenario": "S2"}, {"value": "0.0001016", "module": "C3", "scenario": "S1"}, {"value": "2.553E-07", "module": "C3", "scenario": "S2"}, {"value": "3.811E-08", "module": "C4", "scenario": "S1"}, {"value": "9.461E-05", "module": "C4", "scenario": "S2"}, {"value": "-0.0005062", "module": "D", "scenario": "S1"}, {"value": "-0.000237", "module": "D", "scenario": "S2"}]}}, {"referenceToLCIAMethodDataSet": {"shortDescription": [{"value": "Depletion potential of the stratospheric ozone layer (ODP)", "lang": "en"}, {"value": "Abbau Potential der stratosphärischen Ozonschicht (ODP)", "lang": "de"}], "type": "LCIA method data set", "refObjectId": "b5c629d6-def3-11e6-bf01-fe55135034f3", "uri": "../lciamethods/b5c629d6-def3-11e6-bf01-fe55135034f3.xml"}, "other": {"anies": [{"name": "referenceToUnitGroupDataSet", "value": {"shortDescription": [{"value": "kg CFC11 eq", "lang": "en"}], "type": "unit group data set", "refObjectId": "d9e957c9-7309-4474-bf3a-7777df6c4e5b", "uri": "../unitgroups/d9e957c9-7309-4474-bf3a-7777df6c4e5b.xml"}}, {"value": "3.271E-07", "module": "A1"}, {"value": "2.897E-07", "module": "A2"}, {"value": "4.476E-07", "module": "A3"}, {"value": "9.711E-07", "module": "A4"}, {"value": "1.463E-07", "module": "A5"}, {"value": "0", "module": "B1", "scenario": "S1"}, {"value": "0", "module": "B1", "scenario": "S2"}, {"value": "0", "module": "B2"}, {"value": "0", "module": "B6"}, {"value": "0", "module": "B7"}, {"value": "0", "module": "C1"}, {"value": "1.996E-07", "module": "C2", "scenario": "S1"}, {"value": "4.121E-08", "module": "C2", "scenario": "S2"}, {"value": "7.9E-09", "module": "C3", "scenario": "S1"}, {"value": "5.719E-12", "module": "C3", "scenario": "S2"}, {"value": "8.801E-12", "module": "C4", "scenario": "S1"}, {"value": "4.75E-08", "module": "C4", "scenario": "S2"}, {"value": "-4.538E-08", "module": "D", "scenario": "S1"}, {"value": "-1.338E-08", "module": "D", "scenario": "S2"}]}}, {"referenceToLCIAMethodDataSet": {"shortDescription": [{"value": "Acidification potential of land and water (AP)", "lang": "en"}, {"value": "Versauerungspotenzial von Boden und Wasser (AP)", "lang": "de"}], "type": "LCIA method data set", "refObjectId": "b5c611c6-def3-11e6-bf01-fe55135034f3", "uri": "../lciamethods/b5c611c6-def3-11e6-bf01-fe55135034f3.xml"}, "other": {"anies": [{"name": "referenceToUnitGroupDataSet", "value": {"shortDescription": [{"value": "mol H^(+) eq", "lang": "en"}], "type": "unit group data set", "refObjectId": "42e089ac-92bf-4bf2-8ca1-5fc40d18f2ed", "uri": "../unitgroups/42e089ac-92bf-4bf2-8ca1-5fc40d18f2ed.xml"}}, {"value": "0.01766", "module": "A1"}, {"value": "0.01151", "module": "A2"}, {"value": "0.04283", "module": "A3"}, {"value": "0.1073", "module": "A4"}, {"value": "0.01233", "module": "A5"}, {"value": "0", "module": "B1", "scenario": "S1"}, {"value": "0", "module": "B1", "scenario": "S2"}, {"value": "0", "module": "B2"}, {"value": "0", "module": "B6"}, {"value": "0", "module": "B7"}, {"value": "0", "module": "C1"}, {"value": "0.002446", "module": "C2", "scenario": "S1"}, {"value": "0.000505", "module": "C2", "scenario": "S2"}, {"value": "0.0005557", "module": "C3", "scenario": "S1"}, {"value": "6.323E-07", "module": "C3", "scenario": "S2"}, {"value": "2.486E-07", "module": "C4", "scenario": "S1"}, {"value": "0.001132", "module": "C4", "scenario": "S2"}, {"value": "-0.001602", "module": "D", "scenario": "S1"}, {"value": "-0.0005161", "module": "D", "scenario": "S2"}]}}, {"referenceToLCIAMethodDataSet": {"shortDescription": [{"value": "Eutrophication potential aquatic freshwater (EP-freshwater)", "lang": "en"}, {"value": "Eutrophierungspotenzial Süßwasser (EP-freshwater)", "lang": "de"}], "type": "LCIA method data set", "refObjectId": "b53ec18f-7377-4ad3-86eb-cc3f4f276b2b", "uri": "../lciamethods/b53ec18f-7377-4ad3-86eb-cc3f4f276b2b.xml"}, "other": {"anies": [{"name": "referenceToUnitGroupDataSet", "value": {"shortDescription": [{"value": "kg P eq", "lang": "en"}], "type": "unit group data set", "refObjectId": "0429039d-a61d-4590-ba67-aa4a20a810a1", "uri": "../unitgroups/0429039d-a61d-4590-ba67-aa4a20a810a1.xml"}}, {"value": "9.196E-05", "module": "A1"}, {"value": "1.322E-05", "module": "A2"}, {"value": "0.0001747", "module": "A3"}, {"value": "2.196E-05", "module": "A4"}, {"value": "4.025E-05", "module": "A5"}, {"value": "0", "module": "B1", "scenario": "S1"}, {"value": "0", "module": "B1", "scenario": "S2"}, {"value": "0", "module": "B2"}, {"value": "0", "module": "B6"}, {"value": "0", "module": "B7"}, {"value": "0", "module": "C1"}, {"value": "6.142E-06", "module": "C2", "scenario": "S1"}, {"value": "1.268E-06", "module": "C2", "scenario": "S2"}, {"value": "4.429E-06", "module": "C3", "scenario": "S1"}, {"value": "1.157E-08", "module": "C3", "scenario": "S2"}, {"value": "1.074E-09", "module": "C4", "scenario": "S1"}, {"value": "3.936E-06", "module": "C4", "scenario": "S2"}, {"value": "-1.844E-05", "module": "D", "scenario": "S1"}, {"value": "-6.757E-06", "module": "D", "scenario": "S2"}]}}, {"referenceToLCIAMethodDataSet": {"shortDescription": [{"value": "Eutrophication potential aquatic marine (EP-marine)", "lang": "en"}, {"value": "Eutrophierungspotenzial Salzwasser (EP-marine)", "lang": "de"}], "type": "LCIA method data set", "refObjectId": "b5c619fa-def3-11e6-bf01-fe55135034f3", "uri": "../lciamethods/b5c619fa-def3-11e6-bf01-fe55135034f3.xml"}, "other": {"anies": [{"name": "referenceToUnitGroupDataSet", "value": {"shortDescription": [{"value": "kg N eq", "lang": "en"}], "type": "unit group data set", "refObjectId": "d05bb823-ecdf-4686-8c40-bf1d9257859f", "uri": "../unitgroups/d05bb823-ecdf-4686-8c40-bf1d9257859f.xml"}}, {"value": "0.004464", "module": "A1"}, {"value": "0.004041", "module": "A2"}, {"value": "0.00807", "module": "A3"}, {"value": "0.02621", "module": "A4"}, {"value": "0.002724", "module": "A5"}, {"value": "0", "module": "B1", "scenario": "S1"}, {"value": "0", "module": "B1", "scenario": "S2"}, {"value": "0", "module": "B2"}, {"value": "0", "module": "B6"}, {"value": "0", "module": "B7"}, {"value": "0", "module": "C1"}, {"value": "0.0004861", "module": "C2", "scenario": "S1"}, {"value": "0.0001004", "module": "C2", "scenario": "S2"}, {"value": "0.0001765", "module": "C3", "scenario": "S1"}, {"value": "8.425E-08", "module": "C3", "scenario": "S2"}, {"value": "7.581E-08", "module": "C4", "scenario": "S1"}, {"value": "0.0003865", "module": "C4", "scenario": "S2"}, {"value": "-0.0003723", "module": "D", "scenario": "S1"}, {"value": "-0.0001239", "module": "D", "scenario": "S2"}]}}, {"referenceToLCIAMethodDataSet": {"shortDescription": [{"value": "Eutrophication potential terrestrial (EP-terrestrial)", "lang": "en"}, {"value": "Eutrophierungspotenzial Land (EP-terrestrial)", "lang": "de"}], "type": "LCIA method data set", "refObjectId": "b5c614d2-def3-11e6-bf01-fe55135034f3", "uri": "../lciamethods/b5c614d2-def3-11e6-bf01-fe55135034f3.xml"}, "other": {"anies": [{"name": "referenceToUnitGroupDataSet", "value": {"shortDescription": [{"value": "mol N eq", "lang": "en"}], "type": "unit group data set", "refObjectId": "71b4d617-0ec9-4d3f-b65e-e438940c2401", "uri": "../unitgroups/71b4d617-0ec9-4d3f-b65e-e438940c2401.xml"}}, {"value": "0.05129", "module": "A1"}, {"value": "0.04457", "module": "A2"}, {"value": "0.08786", "module": "A3"}, {"value": "0.2914", "module": "A4"}, {"value": "0.03021", "module": "A5"}, {"value": "0", "module": "B1", "scenario": "S1"}, {"value": "0", "module": "B1", "scenario": "S2"}, {"value": "0", "module": "B2"}, {"value": "0", "module": "B6"}, {"value": "0", "module": "B7"}, {"value": "0", "module": "C1"}, {"value": "0.005418", "module": "C2", "scenario": "S1"}, {"value": "0.001119", "module": "C2", "scenario": "S2"}, {"value": "0.001975", "module": "C3", "scenario": "S1"}, {"value": "9.682E-07", "module": "C3", "scenario": "S2"}, {"value": "8.373E-07", "module": "C4", "scenario": "S1"}, {"value": "0.004265", "module": "C4", "scenario": "S2"}, {"value": "-0.004285", "module": "D", "scenario": "S1"}, {"value": "-0.001415", "module": "D", "scenario": "S2"}]}}, {"referenceToLCIAMethodDataSet": {"shortDescription": [{"value": "Formation potential of tropospheric ozone photochemical oxidants (POCP)", "lang": "en"}, {"value": "Bildungspotential für troposphärisches Ozon (POCP)", "lang": "de"}], "type": "LCIA method data set", "refObjectId": "b5c610fe-def3-11e6-bf01-fe55135034f3", "uri": "../lciamethods/b5c610fe-def3-11e6-bf01-fe55135034f3.xml"}, "other": {"anies": [{"name": "referenceToUnitGroupDataSet", "value": {"shortDescription": [{"value": "kg NMVOC eq", "lang": "en"}], "type": "unit group data set", "refObjectId": "d27c25f8-fbc1-44c6-b47b-4adbae4199c6", "uri": "../unitgroups/d27c25f8-fbc1-44c6-b47b-4adbae4199c6.xml"}}, {"value": "0.01413", "module": "A1"}, {"value": "0.01198", "module": "A2"}, {"value": "0.02521", "module": "A3"}, {"value": "0.07662", "module": "A4"}, {"value": "0.008389", "module": "A5"}, {"value": "0", "module": "B1", "scenario": "S1"}, {"value": "0", "module": "B1", "scenario": "S2"}, {"value": "0", "module": "B2"}, {"value": "0", "module": "B6"}, {"value": "0", "module": "B7"}, {"value": "0", "module": "C1"}, {"value": "0.002083", "module": "C2", "scenario": "S1"}, {"value": "0.0004299", "module": "C2", "scenario": "S2"}, {"value": "0.0005216", "module": "C3", "scenario": "S1"}, {"value": "2.705E-07", "module": "C3", "scenario": "S2"}, {"value": "2.56E-07", "module": "C4", "scenario": "S1"}, {"value": "0.001215", "module": "C4", "scenario": "S2"}, {"value": "-0.001383", "module": "D", "scenario": "S1"}, {"value": "-0.0005852", "module": "D", "scenario": "S2"}]}}, {"referenceToLCIAMethodDataSet": {"shortDescription": [{"value": "Abiotic depletion potential for non fossil resources (ADPE)", "lang": "en"}, {"value": "Potenzial für den abiotischen Abbau nicht fossiler Ressourcen (ADPE)", "lang": "de"}], "type": "LCIA method data set", "refObjectId": "b2ad6494-c78d-11e6-9d9d-cec0c932ce01", "uri": "../lciamethods/b2ad6494-c78d-11e6-9d9d-cec0c932ce01.xml"}, "other": {"anies": [{"name": "referenceToUnitGroupDataSet", "value": {"shortDescription": [{"value": "kg Sb eq", "lang": "en"}], "type": "unit group data set", "refObjectId": "54ccd2d9-a32a-4fc2-923d-f2c8c93e89d4", "uri": "../unitgroups/54ccd2d9-a32a-4fc2-923d-f2c8c93e89d4.xml"}}, {"value": "1.395E-05", "module": "A1"}, {"value": "2.809E-06", "module": "A2"}, {"value": "8.643E-06", "module": "A3"}, {"value": "7.381E-06", "module": "A4"}, {"value": "1.406E-05", "module": "A5"}, {"value": "0", "module": "B1", "scenario": "S1"}, {"value": "0", "module": "B1", "scenario": "S2"}, {"value": "0", "module": "B2"}, {"value": "0", "module": "B6"}, {"value": "0", "module": "B7"}, {"value": "0", "module": "C1"}, {"value": "2.332E-06", "module": "C2", "scenario": "S1"}, {"value": "4.815E-07", "module": "C2", "scenario": "S2"}, {"value": "2.673E-07", "module": "C3", "scenario": "S1"}, {"value": "6.258E-10", "module": "C3", "scenario": "S2"}, {"value": "1.023E-10", "module": "C4", "scenario": "S1"}, {"value": "3.043E-07", "module": "C4", "scenario": "S2"}, {"value": "-1.297E-06", "module": "D", "scenario": "S1"}, {"value": "-2.999E-07", "module": "D", "scenario": "S2"}]}}, {"referenceToLCIAMethodDataSet": {"shortDescription": [{"value": "Abiotic depletion potential for fossil resources (ADPF)", "lang": "en"}, {"value": "Potenzial für den abiotischen Abbau fossiler Brennstoffe (ADPF)", "lang": "de"}], "type": "LCIA method data set", "refObjectId": "b2ad6110-c78d-11e6-9d9d-cec0c932ce01", "uri": "../lciamethods/b2ad6110-c78d-11e6-9d9d-cec0c932ce01.xml"}, "other": {"anies": [{"name": "referenceToUnitGroupDataSet", "value": {"shortDescription": [{"value": "MJ", "lang": "en"}], "type": "unit group data set", "refObjectId": "93a60a57-a3c8-11da-a746-0800200c9a66", "uri": "../unitgroups/93a60a57-a3c8-11da-a746-0800200c9a66.xml"}}, {"value": "35.22", "module": "A1"}, {"value": "19.96", "module": "A2"}, {"value": "104.9", "module": "A3"}, {"value": "62.97", "module": "A4"}, {"value": "18.91", "module": "A5"}, {"value": "0", "module": "B1", "scenario": "S1"}, {"value": "0", "module": "B1", "scenario": "S2"}, {"value": "0", "module": "B2"}, {"value": "0", "module": "B6"}, {"value": "0", "module": "B7"}, {"value": "0", "module": "C1"}, {"value": "13.06", "module": "C2", "scenario": "S1"}, {"value": "2.696", "module": "C2", "scenario": "S2"}, {"value": "1.034", "module": "C3", "scenario": "S1"}, {"value": "0.00231", "module": "C3", "scenario": "S2"}, {"value": "0.0007586", "module": "C4", "scenario": "S1"}, {"value": "3.664", "module": "C4", "scenario": "S2"}, {"value": "-6.912", "module": "D", "scenario": "S1"}, {"value": "-1.824", "module": "D", "scenario": "S2"}]}}, {"referenceToLCIAMethodDataSet": {"shortDescription": [{"value": "Water use (WDP)", "lang": "en"}, {"value": "Wassernutzung (WDP)", "lang": "de"}], "type": "LCIA method data set", "refObjectId": "b2ad66ce-c78d-11e6-9d9d-cec0c932ce01", "uri": "../lciamethods/b2ad66ce-c78d-11e6-9d9d-cec0c932ce01.xml"}, "other": {"anies": [{"name": "referenceToUnitGroupDataSet", "value": {"shortDescription": [{"value": "m^(3) world eq deprived", "lang": "en"}], "type": "unit group data set", "refObjectId": "6ae2df01-888e-46c8-b17d-49fa3869b476", "uri": "../unitgroups/6ae2df01-888e-46c8-b17d-49fa3869b476.xml"}}, {"value": "1.268", "module": "A1"}, {"value": "0.08333", "module": "A2"}, {"value": "0.8334", "module": "A3"}, {"value": "0.1385", "module": "A4"}, {"value": "0.3065", "module": "A5"}, {"value": "0", "module": "B1", "scenario": "S1"}, {"value": "0", "module": "B1", "scenario": "S2"}, {"value": "0", "module": "B2"}, {"value": "0", "module": "B6"}, {"value": "0", "module": "B7"}, {"value": "0", "module": "C1"}, {"value": "0.03975", "module": "C2", "scenario": "S1"}, {"value": "0.008207", "module": "C2", "scenario": "S2"}, {"value": "0.01764", "module": "C3", "scenario": "S1"}, {"value": "2.709E-05", "module": "C3", "scenario": "S2"}, {"value": "-6.448E-06", "module": "C4", "scenario": "S1"}, {"value": "0.01714", "module": "C4", "scenario": "S2"}, {"value": "-0.128", "module": "D", "scenario": "S1"}, {"value": "-0.05823", "module": "D", "scenario": "S2"}]}}, {"referenceToLCIAMethodDataSet": {"shortDescription": [{"value": "Incidence of disease due to PM emissions (PM)", "lang": "en"}, {"value": "Auftreten von Krankheiten aufgrund von Feinstaubemissionen (PM)", "lang": "de"}], "type": "LCIA method data set", "refObjectId": "b5c602c6-def3-11e6-bf01-fe55135034f3", "uri": "../lciamethods/b5c602c6-def3-11e6-bf01-fe55135034f3.xml"}, "other": {"anies": [{"name": "referenceToUnitGroupDataSet", "value": {"shortDescription": [{"value": "Disease incidence", "lang": "en"}], "type": "unit group data set", "refObjectId": "3883559b-648f-4afc-8ba2-0bd24f3affa3", "uri": "../unitgroups/3883559b-648f-4afc-8ba2-0bd24f3affa3.xml"}}, {"value": "1.66E-07", "module": "A1"}, {"value": "8.278E-08", "module": "A2"}, {"value": "5.787E-07", "module": "A3"}, {"value": "2.176E-07", "module": "A4"}, {"value": "9.706E-08", "module": "A5"}, {"value": "0", "module": "B1", "scenario": "S1"}, {"value": "0", "module": "B1", "scenario": "S2"}, {"value": "0", "module": "B2"}, {"value": "0", "module": "B6"}, {"value": "0", "module": "B7"}, {"value": "0", "module": "C1"}, {"value": "6.92E-08", "module": "C2", "scenario": "S1"}, {"value": "1.429E-08", "module": "C2", "scenario": "S2"}, {"value": "4.579E-09", "module": "C3", "scenario": "S1"}, {"value": "2.106E-12", "module": "C3", "scenario": "S2"}, {"value": "6.899E-12", "module": "C4", "scenario": "S1"}, {"value": "2.194E-08", "module": "C4", "scenario": "S2"}, {"value": "-2.3E-08", "module": "D", "scenario": "S1"}, {"value": "-1.139E-08", "module": "D", "scenario": "S2"}]}}, {"referenceToLCIAMethodDataSet": {"shortDescription": [{"value": "Human exposure efficiency relative to U235 (IR)", "lang": "en"}, {"value": "Wirkung durch Exposition des Menschen mit U235 (IR)", "lang": "de"}], "type": "LCIA method data set", "refObjectId": "b5c632be-def3-11e6-bf01-fe55135034f3", "uri": "../lciamethods/b5c632be-def3-11e6-bf01-fe55135034f3.xml"}, "other": {"anies": [{"name": "referenceToUnitGroupDataSet", "value": {"shortDescription": [{"value": "kBq U235 eq", "lang": "en"}], "type": "unit group data set", "refObjectId": "456b05bf-1415-44a9-9993-02452f554c09", "uri": "../unitgroups/456b05bf-1415-44a9-9993-02452f554c09.xml"}}, {"value": "0.13", "module": "A1"}, {"value": "0.08298", "module": "A2"}, {"value": "0.1208", "module": "A3"}, {"value": "0.2707", "module": "A4"}, {"value": "0.05977", "module": "A5"}, {"value": "0", "module": "B1", "scenario": "S1"}, {"value": "0", "module": "B1", "scenario": "S2"}, {"value": "0", "module": "B2"}, {"value": "0", "module": "B6"}, {"value": "0", "module": "B7"}, {"value": "0", "module": "C1"}, {"value": "0.0567", "module": "C2", "scenario": "S1"}, {"value": "0.01171", "module": "C2", "scenario": "S2"}, {"value": "0.007857", "module": "C3", "scenario": "S1"}, {"value": "2.028E-05", "module": "C3", "scenario": "S2"}, {"value": "3.52E-06", "module": "C4", "scenario": "S1"}, {"value": "0.01872", "module": "C4", "scenario": "S2"}, {"value": "-0.03166", "module": "D", "scenario": "S1"}, {"value": "-0.004824", "module": "D", "scenario": "S2"}]}}, {"referenceToLCIAMethodDataSet": {"shortDescription": [{"value": "Comparative toxic unit for ecosystems (ETP-fw)", "lang": "en"}, {"value": "Toxizitätsvergleichseinheit für Ökosysteme (ETP-fw)", "lang": "de"}], "type": "LCIA method data set", "refObjectId": "ee1082d1-b0f7-43ca-a1f0-21e2a4a74511", "uri": "../lciamethods/ee1082d1-b0f7-43ca-a1f0-21e2a4a74511.xml"}, "other": {"anies": [{"name": "referenceToUnitGroupDataSet", "value": {"shortDescription": [{"value": "CTUe", "lang": "en"}], "type": "unit group data set", "refObjectId": "aa959ded-f1eb-4efb-9c5c-2d60be36b3e6", "uri": "../unitgroups/aa959ded-f1eb-4efb-9c5c-2d60be36b3e6.xml"}}, {"value": "104", "module": "A1"}, {"value": "17.16", "module": "A2"}, {"value": "206.3", "module": "A3"}, {"value": "42.53", "module": "A4"}, {"value": "36.36", "module": "A5"}, {"value": "0", "module": "B1", "scenario": "S1"}, {"value": "0", "module": "B1", "scenario": "S2"}, {"value": "0", "module": "B2"}, {"value": "0", "module": "B6"}, {"value": "0", "module": "B7"}, {"value": "0", "module": "C1"}, {"value": "10.25", "module": "C2", "scenario": "S1"}, {"value": "2.116", "module": "C2", "scenario": "S2"}, {"value": "2.184", "module": "C3", "scenario": "S1"}, {"value": "0.00153", "module": "C3", "scenario": "S2"}, {"value": "0.001143", "module": "C4", "scenario": "S1"}, {"value": "2.105", "module": "C4", "scenario": "S2"}, {"value": "-4.843", "module": "D", "scenario": "S1"}, {"value": "-2.597", "module": "D", "scenario": "S2"}]}}, {"referenceToLCIAMethodDataSet": {"shortDescription": [{"value": "Comparative toxic unit for humans (carcinogenic) (HTP-c)", "lang": "en"}, {"value": "Toxizitätsvergleichseinheit für Menschen (krebserregend) (HTP-c)", "lang": "de"}], "type": "LCIA method data set", "refObjectId": "2299222a-bbd8-474f-9d4f-4dd1f18aea7c", "uri": "../lciamethods/2299222a-bbd8-474f-9d4f-4dd1f18aea7c.xml"}, "other": {"anies": [{"name": "referenceToUnitGroupDataSet", "value": {"shortDescription": [{"value": "CTUh", "lang": "en"}], "type": "unit group data set", "refObjectId": "d4c9523e-2d7e-49fd-8469-998f547d3a70", "uri": "../unitgroups/d4c9523e-2d7e-49fd-8469-998f547d3a70.xml"}}, {"value": "1.345E-09", "module": "A1"}, {"value": "6.518E-10", "module": "A2"}, {"value": "3.219E-09", "module": "A3"}, {"value": "2.475E-09", "module": "A4"}, {"value": "1.129E-08", "module": "A5"}, {"value": "0", "module": "B1", "scenario": "S1"}, {"value": "0", "module": "B1", "scenario": "S2"}, {"value": "0", "module": "B2"}, {"value": "0", "module": "B6"}, {"value": "0", "module": "B7"}, {"value": "0", "module": "C1"}, {"value": "3.297E-10", "module": "C2", "scenario": "S1"}, {"value": "6.806E-11", "module": "C2", "scenario": "S2"}, {"value": "2.545E-10", "module": "C3", "scenario": "S1"}, {"value": "7.713E-14", "module": "C3", "scenario": "S2"}, {"value": "6.884E-14", "module": "C4", "scenario": "S1"}, {"value": "6.112E-11", "module": "C4", "scenario": "S2"}, {"value": "-2.843E-11", "module": "D", "scenario": "S1"}, {"value": "8.381E-11", "module": "D", "scenario": "S2"}]}}, {"referenceToLCIAMethodDataSet": {"shortDescription": [{"value": "Comparative toxic unit for humans (noncarcinogenic) (HTP-nc)", "lang": "en"}, {"value": "Toxizitätsvergleichseinheit für Menschen (nicht krebserregend) (HTP-nc)", "lang": "de"}], "type": "LCIA method data set", "refObjectId": "3af763a5-b7a1-48c9-9cee-1f223481fcef", "uri": "../lciamethods/3af763a5-b7a1-48c9-9cee-1f223481fcef.xml"}, "other": {"anies": [{"name": "referenceToUnitGroupDataSet", "value": {"shortDescription": [{"value": "CTUh", "lang": "en"}], "type": "unit group data set", "refObjectId": "d4c9523e-2d7e-49fd-8469-998f547d3a70", "uri": "../unitgroups/d4c9523e-2d7e-49fd-8469-998f547d3a70.xml"}}, {"value": "5.743E-08", "module": "A1"}, {"value": "1.345E-08", "module": "A2"}, {"value": "7.718E-08", "module": "A3"}, {"value": "3.387E-08", "module": "A4"}, {"value": "2.285E-08", "module": "A5"}, {"value": "0", "module": "B1", "scenario": "S1"}, {"value": "0", "module": "B1", "scenario": "S2"}, {"value": "0", "module": "B2"}, {"value": "0", "module": "B6"}, {"value": "0", "module": "B7"}, {"value": "0", "module": "C1"}, {"value": "1.036E-08", "module": "C2", "scenario": "S1"}, {"value": "2.138E-09", "module": "C2", "scenario": "S2"}, {"value": "2.052E-09", "module": "C3", "scenario": "S1"}, {"value": "1.509E-12", "module": "C3", "scenario": "S2"}, {"value": "6.889E-13", "module": "C4", "scenario": "S1"}, {"value": "1.236E-09", "module": "C4", "scenario": "S2"}, {"value": "-1.892E-08", "module": "D", "scenario": "S1"}, {"value": "-1.673E-08", "module": "D", "scenario": "S2"}]}}, {"referenceToLCIAMethodDataSet": {"shortDescription": [{"value": "Soil quality index (SQP)", "lang": "en"}, {"value": "Bodenqualitätsindex (SQP)", "lang": "de"}], "type": "LCIA method data set", "refObjectId": "b2ad6890-c78d-11e6-9d9d-cec0c932ce01", "uri": "../lciamethods/b2ad6890-c78d-11e6-9d9d-cec0c932ce01.xml"}, "other": {"anies": [{"name": "referenceToUnitGroupDataSet", "value": {"shortDescription": [{"value": "SQP", "lang": "en"}], "type": "unit group data set", "refObjectId": "f130951c-e67f-4f7f-8dd4-665de3974e18", "uri": "../unitgroups/f130951c-e67f-4f7f-8dd4-665de3974e18.xml"}}, {"value": "121.2", "module": "A1"}, {"value": "13.59", "module": "A2"}, {"value": "69.54", "module": "A3"}, {"value": "21.05", "module": "A4"}, {"value": "15.23", "module": "A5"}, {"value": "0", "module": "B1", "scenario": "S1"}, {"value": "0", "module": "B1", "scenario": "S2"}, {"value": "0", "module": "B2"}, {"value": "0", "module": "B6"}, {"value": "0", "module": "B7"}, {"value": "0", "module": "C1"}, {"value": "9.102", "module": "C2", "scenario": "S1"}, {"value": "1.879", "module": "C2", "scenario": "S2"}, {"value": "0.5132", "module": "C3", "scenario": "S1"}, {"value": "0.001512", "module": "C3", "scenario": "S2"}, {"value": "0.001179", "module": "C4", "scenario": "S1"}, {"value": "6.909", "module": "C4", "scenario": "S2"}, {"value": "-23.93", "module": "D", "scenario": "S1"}, {"value": "-22.17", "module": "D", "scenario": "S2"}]}}]}, "otherAttributes": {"{http://www.indata.network/EPD/2019}epd-version": "1.2"}, "version": "1.1", "locations": "../ILCDLocations.xml"}