{"processInformation": {"dataSetInformation": {"UUID": "1598f156-ab6f-4419-9381-adc14634997f", "name": {"baseName": [{"value": "Green Roof System", "lang": "en"}, {"value": "Gründachsystem \"Lavendelheide\"", "lang": "de"}], "functionalUnitFlowProperties": [{"lang": "en"}]}, "classificationInformation": {"classification": [{"class": [{"value": "Komposite", "level": 0, "classId": "10"}, {"value": "Systembauteile", "level": 1, "classId": "10.1"}, {"value": "Böden", "level": 2, "classId": "10.1.06"}], "name": "OEKOBAU.DAT"}, {"class": [{"value": "02 Building products", "level": 0}, {"value": "Roof coverings", "level": 1}, {"value": "green roof systems", "level": 2}], "name": "IBUCategories"}]}, "generalComment": [{"value": "A green roof type “Heather with Lavender” serves to offer a permanent habitat on flat and slightly sloping roofs for a certain kind of vegetation, to store water, to discharge excess water and to protect the underlying roof construction. \n\nThe system consists of four or five layers depending on whether the roof to be planted is protected against root penetration or not (see the graphic 1). \n\nIn the case of standard root resistant waterproofing, the Protection Mat SSM 45 is first laid to protect the waterproofing against mechanical damage and to store rainwater. The mat is covered with 40 mm high Floradrain® FD 40 drainage and water storage elements, equipped on the upper side with recesses and channels on the lower side. These elements are in turn covered with the Filter Sheet SF to permanently guarantee the drainage function.\n The Filter Sheet is followed by a layer of System Substrate of at least 100 mm in height. It consists mainly of crushed mineral aggregates and selected organic components.\n The system substrate layer is finally greened by sowing, planting or applying pre-grown vegetation mats; the vegetation itself does not form part of this EPD.\n\nIn exceptional cases of not root resistant waterproofing, the waterproofing is first covered with the Root Barrier WSF 40 or the Root Barrier WSB 100-PO, depending on the roof situation and/or planting, before the Protection Mat SSM 45 is laid.The Root Barriers are not part of this declaration.  \n\n\nKey Graphic 1:\n\n1.0 Roof construction with root resistant waterproofing\n\n\n1.1 Protection Mat SSM 45 \n\n1.2 Floradrain® FD 40 \n\n1.3 Filter Sheet SF \n\n1.4 System Substrate, at least 100 mm thick \n\n1.5 Vegetation\n\n\nProduct according to CPR with ETA \n\nEU regulation no. 305/2011 (CPR) applies for putting the product on the market in the European Union/European Free Trade Association \n\nEU/EFTA (with the exception of Switzerland). The product requires a Declaration of Performance taking into account European Technical Assessment ETA-13/0668 entitled “Kits for Green Roofs” dated 12th June 2018 and CE labelling. \n\nThe respective national regulations apply to use.", "lang": "en"}]}, "quantitativeReference": {"referenceToReferenceFlow": [0]}, "time": {"referenceYear": 2020, "dataSetValidUntil": 2025, "other": {"anies": [{"name": "publicationDateOfEPD", "value": 1596153600000}]}}, "geography": {"locationOfOperationSupplyOrProduction": {"location": "GLO"}}, "technology": {"technologyDescriptionAndIncludedProcesses": [{"value": "A green roof type “Heather with Lavender” serves to offer a permanent habitat on flat and slightly sloping roofs for a certain kind of vegetation, to store water, to discharge excess water and to protect the underlying roof construction. The system consists of four or five layers depending on whether the roof to be planted is protected against root penetration or not (see the graphic 1). In the case of standard root resistant waterproofing, the Protection Mat SSM 45 is first laid to protect the waterproofing against mechanical damage and to store rainwater. The mat is covered with 40 mm high Floradrain® FD 40 drainage and water storage elements, equipped on the upper side with recesses and channels on the lower side. These elements are in turn covered with the Filter Sheet SF to permanently guarantee the drainage function. The Filter Sheet is followed by a layer of System Substrate of at least 100 mm in height. It consists mainly of crushed mineral aggregates and selected organic components. The system substrate layer is finally greened by sowing, planting or applying pre-grown vegetation mats; the vegetation itself does not form part of this EPD. In exceptional cases of not root resistant waterproofing, the waterproofing is first covered with the Root Barrier WSF 40 or the Root Barrier WSB 100-PO, depending on the roof situation and/or planting, before the Protection Mat SSM 45 is laid.The Root Barriers are not part of this declaration. The “Heather with Lavender” green roof system is applied above the usually root resistant waterproofing on sufficiently stable flat or slightly sloping roofs in accordance with the sequence of components described in \"Product description/Product definition”. Roofs greened with this system provide ecological, urban development and constructional benefits such as the creation of new living space for flora and fauna, buffering of areas for microclimate improvement, areas for water retention or urban gardening. \nTechnical data: \nAmongst others, the requirements of European Technical Assessment ETA-13/0668 entitled “Kits for Green Roofs” of 12th June 2018 apply for the “Heather with Lavender” green roof system. The performance characteristics which this assessment requires are shown in the following table: \nDeclared unit: \nThe declared unit is one square meter of installed green roof system without root protection and vegetation layer.", "lang": "en"}, {"value": "Eine Dachbegrünung vom Typ \"Heidekraut mit Lavendel\" dient dazu, auf flachen und leicht geneigten Dächern einen dauerhaften Lebensraum für eine bestimmte Art von Vegetation zu bieten, Wasser zu speichern, überschüssiges Wasser abzuleiten und die darunter liegende Dachkonstruktion zu schützen.\nDas System besteht aus vier oder fünf Schichten, je nachdem, ob das zu begrünende Dach gegen das Eindringen von Wurzeln geschützt ist oder nicht (siehe Grafik 1).\nBei einer wurzelfesten Standardabdichtung wird zunächst die Schutzmatte SSM 45 verlegt, um die Abdichtung vor mechanischen Beschädigungen zu schützen und Regenwasser zu speichern. Die Matte wird mit 40 mm hohen Floradrain® FD 40 Drainage- und Wasserspeicherelementen abgedeckt, die auf der Oberseite mit Aussparungen und Rinnen auf der Unterseite versehen sind. Diese Elemente werden wiederum mit der Filterschicht SF abgedeckt, um die Drainagefunktion dauerhaft zu gewährleisten.\nAuf die Filterschicht folgt eine mindestens 100 mm hohe Schicht aus Systemsubstrat. Sie besteht hauptsächlich aus gebrochenen mineralischen Zuschlagstoffen und ausgewählten organischen Bestandteilen.\nDie Systemsubstratschicht wird abschließend durch Aussaat, Pflanzung oder Aufbringen von vorgewachsenen Vegetationsmatten begrünt; die Vegetation selbst ist nicht Bestandteil dieser EPD.\n\nIn Ausnahmefällen von nicht durchwurzelbaren Abdichtungen wird die Abdichtung je nach Dachsituation und/oder Bepflanzung zunächst mit der Wurzelsperre WSF 40 oder der Wurzelsperre WSB 100-PO abgedeckt, bevor die Schutzmatte SSM 45 verlegt wird; die Wurzelsperren sind nicht Bestandteil dieser Erklärung.\n\nDas Gründachsystem \"Heidekraut mit Lavendel\" wird oberhalb der üblicherweise wurzelfesten Abdichtung auf ausreichend stabilen Flachdächern oder leicht geneigten Dächern gemäß der in \"Produktbeschreibung/Produktdefinition\" beschriebenen Reihenfolge der Komponenten aufgebracht. Mit diesem System begrünte Dächer bieten ökologische, städtebauliche und bauliche Vorteile wie die Schaffung neuer Lebensräume für Flora und Fauna, Pufferung von Flächen zur Verbesserung des Mikroklimas, Flächen zur Wasserrückhaltung oder Urban Gardening. \n", "lang": "de"}], "technologicalApplicability": [{"value": "The “Heather with Lavender” green roof system is applied above the usually root resistant waterproofing on sufficiently stable flat or slightly sloping roofs in accordance with the sequence of components described in \"Product description/Product definition”. Roofs greened with this system provide ecological, urban development and constructional benefits such as the creation of new living space for flora and fauna, buffering of areas for microclimate improvement, areas for water retention or urban gardening.", "lang": "en"}, {"value": "Das Gründachsystem \"Heidekraut mit Lavendel\" wird oberhalb der in der Regel wurzelfesten Abdichtung auf ausreichend stabilen Flachdächern oder leicht geneigten Dächern gemäß der in \"Produktbeschreibung/Produktdefinition\" beschriebenen Komponentenfolge aufgebracht. Mit diesem System begrünte Dächer bieten ökologische, städtebauliche und bauliche Vorteile wie die Schaffung neuer Lebensräume für Flora und Fauna, Pufferung von Flächen zur Verbesserung des Mikroklimas, Flächen zur Wasserrückhaltung oder Urban Gardening.", "lang": "de"}]}}, "modellingAndValidation": {"LCIMethodAndAllocation": {"typeOfDataSet": "EPD", "referenceToLCAMethodDetails": [{"shortDescription": [{"value": "green roof systems.pdf", "lang": "en"}], "type": "source data set", "refObjectId": "84571507-e828-4478-a592-4a712291692f"}], "other": {"anies": [{"name": "subType", "value": "specific dataset"}]}}, "dataSourcesTreatmentAndRepresentativeness": {"referenceToDataSource": [{"shortDescription": [{"value": "GaBi Database (all versions)", "lang": "en"}], "type": "source data set", "refObjectId": "28d74cc0-db8b-4d7e-bc44-5f6d56ce0c4a"}, {"shortDescription": [{"value": "GaBi database SP39 2019", "lang": "en"}], "type": "source data set", "refObjectId": "07d9b8a7-e0fc-408f-a95e-c90735f843ce"}], "useAdviceForDataSet": [{"value": "Scope: \nThis declaration covers the products of  ZinCo GmbH, which is based in Nürtingen. The system components are mainly produced in Germany. The “Heather with Lavender” system, which involves  simple intensive roof greening, was selected as a representative system. Information on further system variants can be obtained from the manufacturer on request. The planting of the green roof system does not  form a part of this declaration. \nSystem boundary: \nCradle to gate with options, modules C1-C4 and D. \n\n\n\nDescription of the system boundaries \n\nModule A1: Manufacturing processes of system components incl. packaging and treatment of manufacturing losses from suppliers.Module A2: Transport  to ZinCo Warehouse.\n\nModule A3: no loads or benefit  \n\nModule A4: Transport to building site (100 km standard distance, needs to be adapted on building level if relevant).\n\nModule A5: Installation of Substrate (by vacuum with Diesel consumption) and treatment of installation losses. Treatment of packaging.\n\nModule B1: Manufacturing of a representative amount of fertilizer (10 grams of nitrogen per year). Emissions are not declared since vegetation is not under study.\n\nModule C1: Deconstruction of the system. Substrate layer is assumed to be vacuumed off the roof (Diesel consumption). All other system components are deconstructed manually (no loads).\n\nModule C2: Transport to EoL treatment (50km standard distance; may be adapted on building level).\n\nModule C3: Thermal treatment of plastics (European Scenario).\n\nModule C4: Disposal of inert and biodegradable waste (European Scenario).\n\nModule D: Benefits & loads beyond the system boundaries.", "lang": "en"}], "other": {"anies": [{"name": "referenceToOriginalEPD", "value": {"shortDescription": {"value": "Green Roof System.pdf", "defaultValue": "Green Roof System.pdf", "lstrings": [{"lang": "en", "value": "Green Roof System.pdf"}]}, "type": "source data set", "uuid": {"uuid": "78f5291f-b439-433a-871b-351b088602e9"}, "refObjectId": "78f5291f-b439-433a-871b-351b088602e9", "resourceURLs": ["https://oekobaudat.de/OEKOBAU.DAT/resource/sources/78f5291f-b439-433a-871b-351b088602e9/Green_Roof_System_12657.pdf?version=00.01.000"]}}]}}, "validation": {"review": [{"referenceToNameOfReviewerAndInstitution": [{"shortDescription": [{"value": "Institut Bauen und Umwelt e. V.", "lang": "en"}], "type": "contact data set", "refObjectId": "d111dbec-b024-4be5-86c5-752d6eb2cf95", "uri": "../contacts/d111dbec-b024-4be5-86c5-752d6eb2cf95.xml"}], "type": "Accredited third party review"}]}, "complianceDeclarations": {"compliance": [{"referenceToComplianceSystem": {"shortDescription": [{"value": "DIN EN 15804+A2", "lang": "en"}], "type": "source data set", "refObjectId": "c0016b33-8cf7-415c-ac6e-deba0d21440d", "uri": "../sources/c0016b33-8cf7-415c-ac6e-deba0d21440d.xml"}}, {"referenceToComplianceSystem": {"shortDescription": [{"value": "ISO 14025", "lang": "en"}], "type": "source data set", "refObjectId": "4f2eb655-6e44-4874-a95a-e28f5442cd4d", "uri": "../sources/4f2eb655-6e44-4874-a95a-e28f5442cd4d.xml"}}]}}, "administrativeInformation": {"commissionerAndGoal": {"referenceToCommissioner": [{"shortDescription": [{"value": "ZinCo GmbH", "lang": "en"}], "type": "contact data set", "refObjectId": "3bab2e51-4052-4004-934b-9ea8a906e242", "uri": "../contacts/3bab2e51-4052-4004-934b-9ea8a906e242.xml"}]}, "dataGenerator": {"referenceToPersonOrEntityGeneratingTheDataSet": [{"shortDescription": [{"value": "Sphera Solutions GmbH", "lang": "en"}], "type": "contact data set", "refObjectId": "623edf96-39d1-4e6f-9892-674c7228546b", "uri": "../contacts/623edf96-39d1-4e6f-9892-674c7228546b.xml"}]}, "dataEntryBy": {"timeStamp": 1596207197208, "referenceToDataSetFormat": [{"shortDescription": [{"value": "ILCD Format", "lang": "en"}], "type": "source data set", "refObjectId": "a97a0155-0234-4b87-b4ce-a45da52f2a40", "uri": "../sources/a97a0155-0234-4b87-b4ce-a45da52f2a40.xml"}, {"shortDescription": [{"value": "EPD-Datenformaterweiterungen v1.2", "lang": "de"}, {"value": "EPD Data Format Extensions v1.2", "lang": "en"}], "type": "source data set", "refObjectId": "a29449fd-aa2f-4de8-b5d7-4b06b43c6fde", "uri": "../sources/a29449fd-aa2f-4de8-b5d7-4b06b43c6fde.xml"}]}, "publicationAndOwnership": {"dataSetVersion": "00.02.000", "referenceToRegistrationAuthority": {"shortDescription": [{"value": "Institut Bauen und Umwelt e. V.", "lang": "en"}], "type": "contact data set", "refObjectId": "d111dbec-b024-4be5-86c5-752d6eb2cf95", "uri": "../contacts/d111dbec-b024-4be5-86c5-752d6eb2cf95.xml"}, "registrationNumber": "EPD-ZIC-20200082-CCA1-EN", "referenceToOwnershipOfDataSet": {"shortDescription": [{"value": "ZinCo GmbH", "lang": "en"}], "type": "contact data set", "refObjectId": "3bab2e51-4052-4004-934b-9ea8a906e242", "uri": "../contacts/3bab2e51-4052-4004-934b-9ea8a906e242.xml"}, "copyright": true, "licenseType": "Free of charge for all users and uses", "accessRestrictions": [{"value": "None", "lang": "en"}], "other": {"anies": [{"name": "referenceToPublisher", "value": {"shortDescription": [{"value": "Institut Bauen und Umwelt e. V.", "lang": "en"}], "type": "contact data set", "refObjectId": "d111dbec-b024-4be5-86c5-752d6eb2cf95", "uri": "../contacts/d111dbec-b024-4be5-86c5-752d6eb2cf95.xml"}}]}}}, "exchanges": {"exchange": [{"dataSetInternalID": 0, "referenceToFlowDataSet": {"shortDescription": [{"value": "\"Heather with Lavender\" Green Roof System (\"Heather with Lavender\" Green Roof System)", "lang": "en"}], "type": "flow data set", "refObjectId": "2b10a4c4-6a13-0225-8da8-7114d8062664", "uri": "../flows/2b10a4c4-6a13-0225-8da8-7114d8062664.xml"}, "meanAmount": 1.0, "referencesToDataSource": {}, "referenceFlow": true, "resolvedFlowVersion": "00.02.000", "resultingflowAmount": 1.0, "flowProperties": [{"name": [{"lang": "en", "value": "Area"}, {"lang": "de", "value": "Fläche"}], "uuid": "93a60a56-a3c8-19da-a746-0800200c9a66", "referenceFlowProperty": true, "meanValue": 1.0, "referenceUnit": "qm", "unitGroupUUID": "c20a03d7-bd90-4569-bc94-66cfd364dfc8"}], "materialProperties": [{"name": "grammage", "value": "102.7035", "unit": "kg/m^2", "unitDescription": "kilograms per square meter"}, {"name": "gross density", "value": "102.7035", "unit": "kg/m^3", "unitDescription": "kilograms per cubic metre"}, {"name": "conversion factor to 1 kg", "value": "102.7035", "unit": "-", "unitDescription": "Without unit"}, {"name": "layer thickness", "value": "0.14", "unit": "m", "unitDescription": "meters"}], "typeOfFlow": "Product flow", "classification": {"classHierarchy": "Komposite / Systembauteile / Böden", "name": "OEKOBAU.DAT"}}, {"dataSetInternalID": 1, "referenceToFlowDataSet": {"shortDescription": [{"value": "Renewable primary energy as energy carrier (PERE)", "lang": "en"}, {"value": "Erneuerbare Primärenergie als Energieträger (PERE)", "lang": "de"}], "type": "flow data set", "refObjectId": "20f32be5-0398-4288-9b6d-accddd195317", "uri": "../flows/20f32be5-0398-4288-9b6d-accddd195317.xml"}, "exchange direction": "INPUT", "other": {"anies": [{"name": "referenceToUnitGroupDataSet", "value": {"shortDescription": [{"value": "MJ", "lang": "en"}], "type": "unit group data set", "refObjectId": "93a60a57-a3c8-11da-a746-0800200c9a66", "uri": "../unitgroups/93a60a57-a3c8-11da-a746-0800200c9a66.xml"}}, {"value": "12.69104", "module": "A1-A3"}, {"value": "0.366436", "module": "A4"}, {"value": "3.68397", "module": "A5"}, {"value": "0.15", "module": "B1"}, {"value": "0.412", "module": "C1"}, {"value": "0.183213", "module": "C2"}, {"value": "0.52163", "module": "C3"}, {"value": "3.12", "module": "C4"}, {"value": "-1.755", "module": "D"}]}, "resolvedFlowVersion": "38.00.000", "flowProperties": [], "typeOfFlow": "Other flow", "classification": {"classHierarchy": "Quantities", "name": "GaBiCategories"}}, {"dataSetInternalID": 2, "referenceToFlowDataSet": {"shortDescription": [{"value": "Renewable primary energy resources as material utilization (PERM)", "lang": "en"}, {"value": "Erneuerbare Primärenergie zur stofflichen Nutzung (PERM)", "lang": "de"}], "type": "flow data set", "refObjectId": "fb3ec0de-548d-4508-aea5-00b73bf6f702", "uri": "../flows/fb3ec0de-548d-4508-aea5-00b73bf6f702.xml"}, "exchange direction": "INPUT", "other": {"anies": [{"name": "referenceToUnitGroupDataSet", "value": {"shortDescription": [{"value": "MJ", "lang": "en"}], "type": "unit group data set", "refObjectId": "93a60a57-a3c8-11da-a746-0800200c9a66", "uri": "../unitgroups/93a60a57-a3c8-11da-a746-0800200c9a66.xml"}}, {"value": "3.24", "module": "A1-A3"}, {"value": "0", "module": "A4"}, {"value": "-3.24", "module": "A5"}, {"value": "0", "module": "B1"}, {"value": "0", "module": "C1"}, {"value": "0", "module": "C2"}, {"value": "0", "module": "C3"}, {"value": "0", "module": "C4"}, {"value": "0", "module": "D"}]}, "resolvedFlowVersion": "38.00.000", "flowProperties": [], "typeOfFlow": "Other flow", "classification": {"classHierarchy": "Quantities", "name": "GaBiCategories"}}, {"dataSetInternalID": 3, "referenceToFlowDataSet": {"shortDescription": [{"value": "Total use of renewable primary energy resources (PERT)", "lang": "en"}, {"value": "Total erneuerbare Primärenergie (PERT)", "lang": "de"}], "type": "flow data set", "refObjectId": "53f97275-fa8a-4cdd-9024-65936002acd0", "uri": "../flows/53f97275-fa8a-4cdd-9024-65936002acd0.xml"}, "exchange direction": "INPUT", "other": {"anies": [{"name": "referenceToUnitGroupDataSet", "value": {"shortDescription": [{"value": "MJ", "lang": "en"}], "type": "unit group data set", "refObjectId": "93a60a57-a3c8-11da-a746-0800200c9a66", "uri": "../unitgroups/93a60a57-a3c8-11da-a746-0800200c9a66.xml"}}, {"value": "15.93104", "module": "A1-A3"}, {"value": "0.366436", "module": "A4"}, {"value": "0.44397", "module": "A5"}, {"value": "0.15", "module": "B1"}, {"value": "0.412", "module": "C1"}, {"value": "0.183213", "module": "C2"}, {"value": "0.52163", "module": "C3"}, {"value": "3.12", "module": "C4"}, {"value": "-1.755", "module": "D"}]}, "resolvedFlowVersion": "38.00.000", "flowProperties": [], "typeOfFlow": "Other flow", "classification": {"classHierarchy": "Quantities / Environmental quantities / EPD EN 15804 / LCI indicators", "name": "GaBiCategories"}}, {"dataSetInternalID": 4, "referenceToFlowDataSet": {"shortDescription": [{"value": "Non renewable primary energy as energy carrier (PENRE)", "lang": "en"}, {"value": "Nicht-erneuerbare Primärenergie als Energieträger (PENRE)", "lang": "de"}], "type": "flow data set", "refObjectId": "ac857178-2b45-46ec-892a-a9a4332f0372", "uri": "../flows/ac857178-2b45-46ec-892a-a9a4332f0372.xml"}, "exchange direction": "INPUT", "other": {"anies": [{"name": "referenceToUnitGroupDataSet", "value": {"shortDescription": [{"value": "MJ", "lang": "en"}], "type": "unit group data set", "refObjectId": "93a60a57-a3c8-11da-a746-0800200c9a66", "uri": "../unitgroups/93a60a57-a3c8-11da-a746-0800200c9a66.xml"}}, {"value": "31.9655", "module": "A1-A3"}, {"value": "6.30369", "module": "A4"}, {"value": "8.751", "module": "A5"}, {"value": "2.04", "module": "B1"}, {"value": "7.08", "module": "C1"}, {"value": "3.14674", "module": "C2"}, {"value": "6.9619", "module": "C3"}, {"value": "37.5", "module": "C4"}, {"value": "-6.256", "module": "D"}]}, "resolvedFlowVersion": "38.00.000", "flowProperties": [], "typeOfFlow": "Other flow", "classification": {"classHierarchy": "Quantities", "name": "GaBiCategories"}}, {"dataSetInternalID": 5, "referenceToFlowDataSet": {"shortDescription": [{"value": "Non renewable primary energy as material utilization (PENRM)", "lang": "en"}, {"value": "Nicht-erneuerbare Primärenergie zur stofflichen Nutzung (PENRM)", "lang": "de"}], "type": "flow data set", "refObjectId": "1421caa0-679d-4bf4-b282-0eb850ccae27", "uri": "../flows/1421caa0-679d-4bf4-b282-0eb850ccae27.xml"}, "exchange direction": "INPUT", "other": {"anies": [{"name": "referenceToUnitGroupDataSet", "value": {"shortDescription": [{"value": "MJ", "lang": "en"}], "type": "unit group data set", "refObjectId": "93a60a57-a3c8-11da-a746-0800200c9a66", "uri": "../unitgroups/93a60a57-a3c8-11da-a746-0800200c9a66.xml"}}, {"value": "14.3026", "module": "A1-A3"}, {"value": "0", "module": "A4"}, {"value": "-1.5026", "module": "A5"}, {"value": "0", "module": "B1"}, {"value": "0", "module": "C1"}, {"value": "0", "module": "C2"}, {"value": "-4.4", "module": "C3"}, {"value": "-8.4", "module": "C4"}, {"value": "0", "module": "D"}]}, "resolvedFlowVersion": "38.00.000", "flowProperties": [], "typeOfFlow": "Other flow", "classification": {"classHierarchy": "Quantities", "name": "GaBiCategories"}}, {"dataSetInternalID": 6, "referenceToFlowDataSet": {"shortDescription": [{"value": "Total use of non renewable primary energy resources (PENRT)", "lang": "en"}, {"value": "Total nicht erneuerbare Primärenergie (PENRT)", "lang": "de"}], "type": "flow data set", "refObjectId": "06159210-646b-4c8d-8583-da9b3b95a6c1", "uri": "../flows/06159210-646b-4c8d-8583-da9b3b95a6c1.xml"}, "exchange direction": "INPUT", "other": {"anies": [{"name": "referenceToUnitGroupDataSet", "value": {"shortDescription": [{"value": "MJ", "lang": "en"}], "type": "unit group data set", "refObjectId": "93a60a57-a3c8-11da-a746-0800200c9a66", "uri": "../unitgroups/93a60a57-a3c8-11da-a746-0800200c9a66.xml"}}, {"value": "46.2681", "module": "A1-A3"}, {"value": "6.30369", "module": "A4"}, {"value": "7.2484", "module": "A5"}, {"value": "2.04", "module": "B1"}, {"value": "7.08", "module": "C1"}, {"value": "3.14674", "module": "C2"}, {"value": "2.5619", "module": "C3"}, {"value": "29.1", "module": "C4"}, {"value": "-6.256", "module": "D"}]}, "resolvedFlowVersion": "38.00.000", "flowProperties": [], "typeOfFlow": "Other flow", "classification": {"classHierarchy": "Quantities / Environmental quantities / EPD EN 15804 / LCI indicators", "name": "GaBiCategories"}}, {"dataSetInternalID": 7, "referenceToFlowDataSet": {"shortDescription": [{"value": "Use of secondary material (SM)", "lang": "en"}, {"value": "Einsatz von Sekundärstoffen (SM)", "lang": "de"}], "type": "flow data set", "refObjectId": "c6a1f35f-2d09-4f54-8dfb-97e502e1ce92", "uri": "../flows/c6a1f35f-2d09-4f54-8dfb-97e502e1ce92.xml"}, "exchange direction": "INPUT", "other": {"anies": [{"name": "referenceToUnitGroupDataSet", "value": {"shortDescription": [{"value": "kg", "lang": "en"}], "type": "unit group data set", "refObjectId": "ad38d542-3fe9-439d-9b95-2f5f7752acaf", "uri": "../unitgroups/ad38d542-3fe9-439d-9b95-2f5f7752acaf.xml"}}, {"value": "52.759", "module": "A1-A3"}, {"value": "0", "module": "A4"}, {"value": "0", "module": "A5"}, {"value": "0", "module": "B1"}, {"value": "0", "module": "C1"}, {"value": "0", "module": "C2"}, {"value": "0", "module": "C3"}, {"value": "0", "module": "C4"}, {"value": "0", "module": "D"}]}, "resolvedFlowVersion": "38.00.000", "flowProperties": [], "typeOfFlow": "Other flow", "classification": {"classHierarchy": "Quantities / Environmental quantities / EPD EN 15804 / LCI indicators", "name": "GaBiCategories"}}, {"dataSetInternalID": 8, "referenceToFlowDataSet": {"shortDescription": [{"value": "Use of renewable secondary fuels (RSF)", "lang": "en"}, {"value": "Erneuerbare Sekundärbrennstoffe (RSF)", "lang": "de"}], "type": "flow data set", "refObjectId": "64333088-a55f-4aa2-9a31-c10b07816787", "uri": "../flows/64333088-a55f-4aa2-9a31-c10b07816787.xml"}, "exchange direction": "INPUT", "other": {"anies": [{"name": "referenceToUnitGroupDataSet", "value": {"shortDescription": [{"value": "MJ", "lang": "en"}], "type": "unit group data set", "refObjectId": "93a60a57-a3c8-11da-a746-0800200c9a66", "uri": "../unitgroups/93a60a57-a3c8-11da-a746-0800200c9a66.xml"}}, {"value": "0", "module": "A1-A3"}, {"value": "0", "module": "A4"}, {"value": "0", "module": "A5"}, {"value": "0", "module": "B1"}, {"value": "0", "module": "C1"}, {"value": "0", "module": "C2"}, {"value": "0", "module": "C3"}, {"value": "0", "module": "C4"}, {"value": "0", "module": "D"}]}, "resolvedFlowVersion": "38.00.000", "flowProperties": [], "typeOfFlow": "Other flow", "classification": {"classHierarchy": "Quantities / Environmental quantities / EPD EN 15804 / LCI indicators", "name": "GaBiCategories"}}, {"dataSetInternalID": 9, "referenceToFlowDataSet": {"shortDescription": [{"value": "Use of non renewable secondary fuels (NRSF)", "lang": "en"}, {"value": "Nicht erneuerbare Sekundärbrennstoffe (NRSF)", "lang": "de"}], "type": "flow data set", "refObjectId": "89def144-d39a-4287-b86f-efde453ddcb2", "uri": "../flows/89def144-d39a-4287-b86f-efde453ddcb2.xml"}, "exchange direction": "INPUT", "other": {"anies": [{"name": "referenceToUnitGroupDataSet", "value": {"shortDescription": [{"value": "MJ", "lang": "en"}], "type": "unit group data set", "refObjectId": "93a60a57-a3c8-11da-a746-0800200c9a66", "uri": "../unitgroups/93a60a57-a3c8-11da-a746-0800200c9a66.xml"}}, {"value": "0", "module": "A1-A3"}, {"value": "0", "module": "A4"}, {"value": "0", "module": "A5"}, {"value": "0", "module": "B1"}, {"value": "0", "module": "C1"}, {"value": "0", "module": "C2"}, {"value": "0", "module": "C3"}, {"value": "0", "module": "C4"}, {"value": "0", "module": "D"}]}, "resolvedFlowVersion": "38.00.000", "flowProperties": [], "typeOfFlow": "Other flow", "classification": {"classHierarchy": "Quantities / Environmental quantities / EPD EN 15804 / LCI indicators", "name": "GaBiCategories"}}, {"dataSetInternalID": 10, "referenceToFlowDataSet": {"shortDescription": [{"value": "Use of net fresh water (FW)", "lang": "en"}, {"value": "Einsatz von Süßwasserressourcen (FW)", "lang": "de"}], "type": "flow data set", "refObjectId": "3cf952c8-f3a4-461d-8c96-96456ca62246", "uri": "../flows/3cf952c8-f3a4-461d-8c96-96456ca62246.xml"}, "exchange direction": "INPUT", "other": {"anies": [{"name": "referenceToUnitGroupDataSet", "value": {"shortDescription": [{"value": "m^3", "lang": "en"}], "type": "unit group data set", "refObjectId": "cd950537-0a98-4044-9ba7-9f9a68d0a504", "uri": "../unitgroups/cd950537-0a98-4044-9ba7-9f9a68d0a504.xml"}}, {"value": "0.00693967", "module": "A1-A3"}, {"value": "0.000328133", "module": "A4"}, {"value": "0.001905", "module": "A5"}, {"value": "0.000634", "module": "B1"}, {"value": "0.000369", "module": "C1"}, {"value": "0.000164567", "module": "C2"}, {"value": "0.016795", "module": "C3"}, {"value": "0.00551", "module": "C4"}, {"value": "-0.002028", "module": "D"}]}, "resolvedFlowVersion": "38.00.000", "flowProperties": [], "typeOfFlow": "Other flow", "classification": {"classHierarchy": "Quantities / Environmental quantities / EPD EN 15804 / LCI indicators", "name": "GaBiCategories"}}, {"dataSetInternalID": 11, "referenceToFlowDataSet": {"shortDescription": [{"value": "Hazardous waste disposed (HWD)", "lang": "en"}, {"value": "Gefährlicher Abfall zur Deponie (HWD)", "lang": "de"}], "type": "flow data set", "refObjectId": "430f9e0f-59b2-46a0-8e0d-55e0e84948fc", "uri": "../flows/430f9e0f-59b2-46a0-8e0d-55e0e84948fc.xml"}, "exchange direction": "OUTPUT", "other": {"anies": [{"name": "referenceToUnitGroupDataSet", "value": {"shortDescription": [{"value": "kg", "lang": "en"}], "type": "unit group data set", "refObjectId": "ad38d542-3fe9-439d-9b95-2f5f7752acaf", "uri": "../unitgroups/ad38d542-3fe9-439d-9b95-2f5f7752acaf.xml"}}, {"value": "4.50902E-07", "module": "A1-A3"}, {"value": "2.35985E-07", "module": "A4"}, {"value": "2.653094E-07", "module": "A5"}, {"value": "1.66E-09", "module": "B1"}, {"value": "2.65E-07", "module": "C1"}, {"value": "1.1799E-07", "module": "C2"}, {"value": "8.5783E-09", "module": "C3"}, {"value": "3.12E-07", "module": "C4"}, {"value": "-2.523E-09", "module": "D"}]}, "resolvedFlowVersion": "38.00.000", "flowProperties": [], "typeOfFlow": "Other flow", "classification": {"classHierarchy": "Quantities / Environmental quantities / EPD EN 15804 / LCI indicators", "name": "GaBiCategories"}}, {"dataSetInternalID": 12, "referenceToFlowDataSet": {"shortDescription": [{"value": "Non hazardous waste disposed (NHWD)", "lang": "en"}, {"value": "Entsorgter nicht gefährlicher Abfall (NHWD)", "lang": "de"}], "type": "flow data set", "refObjectId": "b29ef66b-e286-4afa-949f-62f1a7b4d7fa", "uri": "../flows/b29ef66b-e286-4afa-949f-62f1a7b4d7fa.xml"}, "exchange direction": "OUTPUT", "other": {"anies": [{"name": "referenceToUnitGroupDataSet", "value": {"shortDescription": [{"value": "kg", "lang": "en"}], "type": "unit group data set", "refObjectId": "ad38d542-3fe9-439d-9b95-2f5f7752acaf", "uri": "../unitgroups/ad38d542-3fe9-439d-9b95-2f5f7752acaf.xml"}}, {"value": "0.21021436", "module": "A1-A3"}, {"value": "0.00110747", "module": "A4"}, {"value": "0.02311", "module": "A5"}, {"value": "0.215", "module": "B1"}, {"value": "0.00124", "module": "C1"}, {"value": "0.000552783", "module": "C2"}, {"value": "0.62736", "module": "C3"}, {"value": "98.3", "module": "C4"}, {"value": "-0.003319", "module": "D"}]}, "resolvedFlowVersion": "38.00.000", "flowProperties": [], "typeOfFlow": "Other flow", "classification": {"classHierarchy": "Quantities / Environmental quantities / EPD EN 15804 / LCI indicators", "name": "GaBiCategories"}}, {"dataSetInternalID": 13, "referenceToFlowDataSet": {"shortDescription": [{"value": "Radioactive waste disposed (RWD)", "lang": "en"}, {"value": "Entsorgter radioaktiver Abfall (RWD)", "lang": "de"}], "type": "flow data set", "refObjectId": "3449546e-52ad-4b39-b809-9fb77cea8ff6", "uri": "../flows/3449546e-52ad-4b39-b809-9fb77cea8ff6.xml"}, "exchange direction": "OUTPUT", "other": {"anies": [{"name": "referenceToUnitGroupDataSet", "value": {"shortDescription": [{"value": "kg", "lang": "en"}], "type": "unit group data set", "refObjectId": "ad38d542-3fe9-439d-9b95-2f5f7752acaf", "uri": "../unitgroups/ad38d542-3fe9-439d-9b95-2f5f7752acaf.xml"}}, {"value": "0.0011775844", "module": "A1-A3"}, {"value": "6.63515E-06", "module": "A4"}, {"value": "1.547E-05", "module": "A5"}, {"value": "2.45E-05", "module": "B1"}, {"value": "7.46E-06", "module": "C1"}, {"value": "3.31237E-06", "module": "C2"}, {"value": "0.00010605", "module": "C3"}, {"value": "0.000339", "module": "C4"}, {"value": "-0.0006006", "module": "D"}]}, "resolvedFlowVersion": "38.00.000", "flowProperties": [], "typeOfFlow": "Other flow", "classification": {"classHierarchy": "Quantities / Environmental quantities / EPD EN 15804 / LCI indicators", "name": "GaBiCategories"}}, {"dataSetInternalID": 14, "referenceToFlowDataSet": {"shortDescription": [{"value": "Components for re-use (CRU)", "lang": "en"}, {"value": "Komponenten für die Wiederverwendung (CRU)", "lang": "de"}], "type": "flow data set", "refObjectId": "a2b32f97-3fc7-4af2-b209-525bc6426f33", "uri": "../flows/a2b32f97-3fc7-4af2-b209-525bc6426f33.xml"}, "exchange direction": "OUTPUT", "other": {"anies": [{"name": "referenceToUnitGroupDataSet", "value": {"shortDescription": [{"value": "kg", "lang": "en"}], "type": "unit group data set", "refObjectId": "ad38d542-3fe9-439d-9b95-2f5f7752acaf", "uri": "../unitgroups/ad38d542-3fe9-439d-9b95-2f5f7752acaf.xml"}}, {"value": "0", "module": "A1-A3"}, {"value": "0", "module": "A4"}, {"value": "0", "module": "A5"}, {"value": "0", "module": "B1"}, {"value": "0", "module": "C1"}, {"value": "0", "module": "C2"}, {"value": "0", "module": "C3"}, {"value": "0", "module": "C4"}, {"value": "0", "module": "D"}]}, "resolvedFlowVersion": "38.00.000", "flowProperties": [], "typeOfFlow": "Other flow", "classification": {"classHierarchy": "Quantities / Environmental quantities / EPD EN 15804 / LCI indicators", "name": "GaBiCategories"}}, {"dataSetInternalID": 15, "referenceToFlowDataSet": {"shortDescription": [{"value": "Materials for recycling (MFR)", "lang": "en"}, {"value": "Stoffe zum Recycling (MFR)", "lang": "de"}], "type": "flow data set", "refObjectId": "d7fe48a5-4103-49c8-9aae-b0b5dfdbd6ae", "uri": "../flows/d7fe48a5-4103-49c8-9aae-b0b5dfdbd6ae.xml"}, "exchange direction": "OUTPUT", "other": {"anies": [{"name": "referenceToUnitGroupDataSet", "value": {"shortDescription": [{"value": "kg", "lang": "en"}], "type": "unit group data set", "refObjectId": "ad38d542-3fe9-439d-9b95-2f5f7752acaf", "uri": "../unitgroups/ad38d542-3fe9-439d-9b95-2f5f7752acaf.xml"}}, {"value": "0", "module": "A1-A3"}, {"value": "0", "module": "A4"}, {"value": "0", "module": "A5"}, {"value": "0", "module": "B1"}, {"value": "0", "module": "C1"}, {"value": "0", "module": "C2"}, {"value": "0", "module": "C3"}, {"value": "0", "module": "C4"}, {"value": "0", "module": "D"}]}, "resolvedFlowVersion": "38.00.000", "flowProperties": [], "typeOfFlow": "Other flow", "classification": {"classHierarchy": "Quantities / Environmental quantities / EPD EN 15804 / LCI indicators", "name": "GaBiCategories"}}, {"dataSetInternalID": 16, "referenceToFlowDataSet": {"shortDescription": [{"value": "Materials for energy recovery (MER)", "lang": "en"}, {"value": "Stoffe für die Energierückgewinnung (MER)", "lang": "de"}], "type": "flow data set", "refObjectId": "59a9181c-3aaf-46ee-8b13-2b3723b6e447", "uri": "../flows/59a9181c-3aaf-46ee-8b13-2b3723b6e447.xml"}, "exchange direction": "OUTPUT", "other": {"anies": [{"name": "referenceToUnitGroupDataSet", "value": {"shortDescription": [{"value": "kg", "lang": "en"}], "type": "unit group data set", "refObjectId": "ad38d542-3fe9-439d-9b95-2f5f7752acaf", "uri": "../unitgroups/ad38d542-3fe9-439d-9b95-2f5f7752acaf.xml"}}, {"value": "0", "module": "A1-A3"}, {"value": "0", "module": "A4"}, {"value": "0", "module": "A5"}, {"value": "0", "module": "B1"}, {"value": "0", "module": "C1"}, {"value": "0", "module": "C2"}, {"value": "0", "module": "C3"}, {"value": "0", "module": "C4"}, {"value": "0", "module": "D"}]}, "resolvedFlowVersion": "38.00.000", "flowProperties": [], "typeOfFlow": "Other flow", "classification": {"classHierarchy": "Quantities / Environmental quantities / EPD EN 15804 / LCI indicators", "name": "GaBiCategories"}}, {"dataSetInternalID": 17, "referenceToFlowDataSet": {"shortDescription": [{"value": "Exported electrical energy (EEE)", "lang": "en"}, {"value": "Exportierte elektrische Energie (EEE)", "lang": "de"}], "type": "flow data set", "refObjectId": "4da0c987-2b76-40d6-9e9e-82a017aaaf29", "uri": "../flows/4da0c987-2b76-40d6-9e9e-82a017aaaf29.xml"}, "exchange direction": "OUTPUT", "other": {"anies": [{"name": "referenceToUnitGroupDataSet", "value": {"shortDescription": [{"value": "MJ", "lang": "en"}], "type": "unit group data set", "refObjectId": "93a60a57-a3c8-11da-a746-0800200c9a66", "uri": "../unitgroups/93a60a57-a3c8-11da-a746-0800200c9a66.xml"}}, {"value": "0", "module": "A1-A3"}, {"value": "0", "module": "A4"}, {"value": "1.157", "module": "A5"}, {"value": "0", "module": "B1"}, {"value": "0", "module": "C1"}, {"value": "0", "module": "C2"}, {"value": "15.065", "module": "C3"}, {"value": "2.71", "module": "C4"}, {"value": "0", "module": "D"}]}, "resolvedFlowVersion": "38.00.000", "flowProperties": [], "typeOfFlow": "Other flow", "classification": {"classHierarchy": "Quantities / Environmental quantities / EPD EN 15804 / LCI indicators", "name": "GaBiCategories"}}, {"dataSetInternalID": 18, "referenceToFlowDataSet": {"shortDescription": [{"value": "Exported thermal energy (EET)", "lang": "en"}, {"value": "Exportierte thermische Energie (EET)", "lang": "de"}], "type": "flow data set", "refObjectId": "98daf38a-7a79-46d3-9a37-2b7bd0955810", "uri": "../flows/98daf38a-7a79-46d3-9a37-2b7bd0955810.xml"}, "exchange direction": "OUTPUT", "other": {"anies": [{"name": "referenceToUnitGroupDataSet", "value": {"shortDescription": [{"value": "MJ", "lang": "en"}], "type": "unit group data set", "refObjectId": "93a60a57-a3c8-11da-a746-0800200c9a66", "uri": "../unitgroups/93a60a57-a3c8-11da-a746-0800200c9a66.xml"}}, {"value": "0", "module": "A1-A3"}, {"value": "0", "module": "A4"}, {"value": "2.079", "module": "A5"}, {"value": "0", "module": "B1"}, {"value": "0", "module": "C1"}, {"value": "0", "module": "C2"}, {"value": "27.24", "module": "C3"}, {"value": "0", "module": "C4"}, {"value": "0", "module": "D"}]}, "resolvedFlowVersion": "38.00.000", "flowProperties": [], "typeOfFlow": "Other flow", "classification": {"classHierarchy": "Quantities / Environmental quantities / EPD EN 15804 / LCI indicators", "name": "GaBiCategories"}}]}, "LCIAResults": {"LCIAResult": [{"referenceToLCIAMethodDataSet": {"shortDescription": [{"value": "Global Warming Potential total (GWP-total)", "lang": "en"}, {"value": "Globales Erwärmungspotenzial total (GWP-total)", "lang": "de"}], "type": "LCIA method data set", "refObjectId": "6a37f984-a4b3-458a-a20a-64418c145fa2", "uri": "../lciamethods/6a37f984-a4b3-458a-a20a-64418c145fa2.xml"}, "other": {"anies": [{"name": "referenceToUnitGroupDataSet", "value": {"shortDescription": [{"value": "kg CO_(2)-Äq.", "lang": "en"}], "type": "unit group data set", "refObjectId": "1ebf3012-d0db-4de2-aefd-ef30cedb0be1", "uri": "../unitgroups/1ebf3012-d0db-4de2-aefd-ef30cedb0be1.xml"}}, {"value": "-2.67363", "module": "A1-A3"}, {"value": "0.476208", "module": "A4"}, {"value": "0.694", "module": "A5"}, {"value": "0.0994", "module": "B1"}, {"value": "0.0512", "module": "C1"}, {"value": "0.238089", "module": "C2"}, {"value": "6.845", "module": "C3"}, {"value": "11.5", "module": "C4"}, {"value": "-0.3663", "module": "D"}]}}, {"referenceToLCIAMethodDataSet": {"shortDescription": [{"value": "Global Warming Potential fossil fuels (GWP-fossil)", "lang": "en"}, {"value": "Globales Erwärmungspotenzial fossil (GWP-fossil)", "lang": "de"}], "type": "LCIA method data set", "refObjectId": "5f635281-343e-44fb-83df-1971b155e6b6", "uri": "../lciamethods/5f635281-343e-44fb-83df-1971b155e6b6.xml"}, "other": {"anies": [{"name": "referenceToUnitGroupDataSet", "value": {"shortDescription": [{"value": "kg CO_(2)-Äq.", "lang": "en"}], "type": "unit group data set", "refObjectId": "1ebf3012-d0db-4de2-aefd-ef30cedb0be1", "uri": "../unitgroups/1ebf3012-d0db-4de2-aefd-ef30cedb0be1.xml"}}, {"value": "2.64195", "module": "A1-A3"}, {"value": "0.474095", "module": "A4"}, {"value": "0.3917", "module": "A5"}, {"value": "0.0965", "module": "B1"}, {"value": "0.0726", "module": "C1"}, {"value": "0.237048", "module": "C2"}, {"value": "6.845", "module": "C3"}, {"value": "2.17", "module": "C4"}, {"value": "-0.3656", "module": "D"}]}}, {"referenceToLCIAMethodDataSet": {"shortDescription": [{"value": "Global Warming Potential biogenic (GWP-biogenic)", "lang": "en"}, {"value": "Globales Erwärmungspotenzial biogen (GWP-biogenic)", "lang": "de"}], "type": "LCIA method data set", "refObjectId": "2356e1ab-0185-4db5-86e5-16de51c7485c", "uri": "../lciamethods/2356e1ab-0185-4db5-86e5-16de51c7485c.xml"}, "other": {"anies": [{"name": "referenceToUnitGroupDataSet", "value": {"shortDescription": [{"value": "kg CO_(2)-Äq.", "lang": "en"}], "type": "unit group data set", "refObjectId": "1ebf3012-d0db-4de2-aefd-ef30cedb0be1", "uri": "../unitgroups/1ebf3012-d0db-4de2-aefd-ef30cedb0be1.xml"}}, {"value": "-5.318363101", "module": "A1-A3"}, {"value": "0.000190463", "module": "A4"}, {"value": "0.3004", "module": "A5"}, {"value": "0.00282", "module": "B1"}, {"value": "-0.0236", "module": "C1"}, {"value": "9.5432E-05", "module": "C2"}, {"value": "-0.00031568", "module": "C3"}, {"value": "9.31", "module": "C4"}, {"value": "-0.000954", "module": "D"}]}}, {"referenceToLCIAMethodDataSet": {"shortDescription": [{"value": "Global Warming Potential luluc (GWP-luluc)", "lang": "en"}, {"value": "Globales Erwärmungspotenzial luluc (GWP-luluc)", "lang": "de"}], "type": "LCIA method data set", "refObjectId": "4331bbdb-978a-490d-8707-eeb047f01a55", "uri": "../lciamethods/4331bbdb-978a-490d-8707-eeb047f01a55.xml"}, "other": {"anies": [{"name": "referenceToUnitGroupDataSet", "value": {"shortDescription": [{"value": "kg CO_(2)-Äq.", "lang": "en"}], "type": "unit group data set", "refObjectId": "1ebf3012-d0db-4de2-aefd-ef30cedb0be1", "uri": "../unitgroups/1ebf3012-d0db-4de2-aefd-ef30cedb0be1.xml"}}, {"value": "0.006426", "module": "A1-A3"}, {"value": "0.00198734", "module": "A4"}, {"value": "0.00224013", "module": "A5"}, {"value": "7.05E-05", "module": "B1"}, {"value": "0.00223", "module": "C1"}, {"value": "0.00099261", "module": "C2"}, {"value": "0.00023028", "module": "C3"}, {"value": "0.00453", "module": "C4"}, {"value": "-0.0003291", "module": "D"}]}}, {"referenceToLCIAMethodDataSet": {"shortDescription": [{"value": "Depletion potential of the stratospheric ozone layer (ODP)", "lang": "en"}, {"value": "Abbau Potential der stratosphärischen Ozonschicht (ODP)", "lang": "de"}], "type": "LCIA method data set", "refObjectId": "b5c629d6-def3-11e6-bf01-fe55135034f3", "uri": "../lciamethods/b5c629d6-def3-11e6-bf01-fe55135034f3.xml"}, "other": {"anies": [{"name": "referenceToUnitGroupDataSet", "value": {"shortDescription": [{"value": "kg CFC11-Äq.", "lang": "en"}], "type": "unit group data set", "refObjectId": "d9e957c9-7309-4474-bf3a-7777df6c4e5b", "uri": "../unitgroups/d9e957c9-7309-4474-bf3a-7777df6c4e5b.xml"}}, {"value": "3.3682533E-14", "module": "A1-A3"}, {"value": "1.15941E-16", "module": "A4"}, {"value": "2.36E-16", "module": "A5"}, {"value": "6.16E-16", "module": "B1"}, {"value": "1.31E-16", "module": "C1"}, {"value": "5.81703E-17", "module": "C2"}, {"value": "1.9131E-15", "module": "C3"}, {"value": "6.81E-15", "module": "C4"}, {"value": "-4.944E-15", "module": "D"}]}}, {"referenceToLCIAMethodDataSet": {"shortDescription": [{"value": "Acidification potential of land and water (AP)", "lang": "en"}, {"value": "Versauerungspotenzial von Boden und Wasser (AP)", "lang": "de"}], "type": "LCIA method data set", "refObjectId": "b5c611c6-def3-11e6-bf01-fe55135034f3", "uri": "../lciamethods/b5c611c6-def3-11e6-bf01-fe55135034f3.xml"}, "other": {"anies": [{"name": "referenceToUnitGroupDataSet", "value": {"shortDescription": [{"value": "mol H^(+)-Äq.", "lang": "en"}], "type": "unit group data set", "refObjectId": "42e089ac-92bf-4bf2-8ca1-5fc40d18f2ed", "uri": "../unitgroups/42e089ac-92bf-4bf2-8ca1-5fc40d18f2ed.xml"}}, {"value": "0.00597063", "module": "A1-A3"}, {"value": "0.000394429", "module": "A4"}, {"value": "0.0003722", "module": "A5"}, {"value": "0.000694", "module": "B1"}, {"value": "0.000287", "module": "C1"}, {"value": "0.000197235", "module": "C2"}, {"value": "0.0008967", "module": "C3"}, {"value": "0.0131", "module": "C4"}, {"value": "-0.0005902", "module": "D"}]}}, {"referenceToLCIAMethodDataSet": {"shortDescription": [{"value": "Eutrophication potential aquatic freshwater (EP-freshwater)", "lang": "en"}, {"value": "Eutrophierungspotenzial Süßwasser (EP-freshwater)", "lang": "de"}], "type": "LCIA method data set", "refObjectId": "b53ec18f-7377-4ad3-86eb-cc3f4f276b2b", "uri": "../lciamethods/b53ec18f-7377-4ad3-86eb-cc3f4f276b2b.xml"}, "other": {"anies": [{"name": "referenceToUnitGroupDataSet", "value": {"shortDescription": [{"value": "kg PO_(4)-Äq.", "lang": "en"}], "type": "unit group data set", "refObjectId": "0429039d-a61d-4590-ba67-aa4a20a810a1", "uri": "../unitgroups/0429039d-a61d-4590-ba67-aa4a20a810a1.xml"}}, {"value": "8.14666E-06", "module": "A1-A3"}, {"value": "1.03301E-06", "module": "A4"}, {"value": "1.17571E-06", "module": "A5"}, {"value": "2.26E-06", "module": "B1"}, {"value": "1.16E-06", "module": "C1"}, {"value": "5.16512E-07", "module": "C2"}, {"value": "3.2209E-07", "module": "C3"}, {"value": "0.000458", "module": "C4"}, {"value": "-6.058E-07", "module": "D"}]}}, {"referenceToLCIAMethodDataSet": {"shortDescription": [{"value": "Eutrophication potential aquatic marine (EP-marine)", "lang": "en"}, {"value": "Eutrophierungspotenzial Salzwasser (EP-marine)", "lang": "de"}], "type": "LCIA method data set", "refObjectId": "b5c619fa-def3-11e6-bf01-fe55135034f3", "uri": "../lciamethods/b5c619fa-def3-11e6-bf01-fe55135034f3.xml"}, "other": {"anies": [{"name": "referenceToUnitGroupDataSet", "value": {"shortDescription": [{"value": "kg N-Äq.", "lang": "en"}], "type": "unit group data set", "refObjectId": "d05bb823-ecdf-4686-8c40-bf1d9257859f", "uri": "../unitgroups/d05bb823-ecdf-4686-8c40-bf1d9257859f.xml"}}, {"value": "0.00243465", "module": "A1-A3"}, {"value": "0.000113404", "module": "A4"}, {"value": "7.415E-05", "module": "A5"}, {"value": "8.21E-05", "module": "B1"}, {"value": "4.94E-05", "module": "C1"}, {"value": "5.65017E-05", "module": "C2"}, {"value": "0.00024063", "module": "C3"}, {"value": "0.00655", "module": "C4"}, {"value": "-0.000145", "module": "D"}]}}, {"referenceToLCIAMethodDataSet": {"shortDescription": [{"value": "Eutrophication potential terrestrial (EP-terrestrial)", "lang": "en"}, {"value": "Eutrophierungspotenzial Land (EP-terrestrial)", "lang": "de"}], "type": "LCIA method data set", "refObjectId": "b5c614d2-def3-11e6-bf01-fe55135034f3", "uri": "../lciamethods/b5c614d2-def3-11e6-bf01-fe55135034f3.xml"}, "other": {"anies": [{"name": "referenceToUnitGroupDataSet", "value": {"shortDescription": [{"value": "mol N-Äq.", "lang": "en"}], "type": "unit group data set", "refObjectId": "71b4d617-0ec9-4d3f-b65e-e438940c2401", "uri": "../unitgroups/71b4d617-0ec9-4d3f-b65e-e438940c2401.xml"}}, {"value": "0.02679029", "module": "A1-A3"}, {"value": "0.0013938", "module": "A4"}, {"value": "0.0010949", "module": "A5"}, {"value": "0.000894", "module": "B1"}, {"value": "0.000701", "module": "C1"}, {"value": "0.0006989", "module": "C2"}, {"value": "0.004014", "module": "C3"}, {"value": "0.0383", "module": "C4"}, {"value": "-0.001542", "module": "D"}]}}, {"referenceToLCIAMethodDataSet": {"shortDescription": [{"value": "Formation potential of tropospheric ozone photochemical oxidants (POCP)", "lang": "en"}, {"value": "Bildungspotential für troposphärisches Ozon (POCP)", "lang": "de"}], "type": "LCIA method data set", "refObjectId": "b5c610fe-def3-11e6-bf01-fe55135034f3", "uri": "../lciamethods/b5c610fe-def3-11e6-bf01-fe55135034f3.xml"}, "other": {"anies": [{"name": "referenceToUnitGroupDataSet", "value": {"shortDescription": [{"value": "kg NMVOC-Äq.", "lang": "en"}], "type": "unit group data set", "refObjectId": "d27c25f8-fbc1-44c6-b47b-4adbae4199c6", "uri": "../unitgroups/d27c25f8-fbc1-44c6-b47b-4adbae4199c6.xml"}}, {"value": "0.006392578", "module": "A1-A3"}, {"value": "0.000315842", "module": "A4"}, {"value": "0.0002645", "module": "A5"}, {"value": "0.000258", "module": "B1"}, {"value": "0.000195", "module": "C1"}, {"value": "0.000157921", "module": "C2"}, {"value": "0.0006896", "module": "C3"}, {"value": "0.0133", "module": "C4"}, {"value": "-0.0004103", "module": "D"}]}}, {"referenceToLCIAMethodDataSet": {"shortDescription": [{"value": "Abiotic depletion potential for non fossil resources (ADPE)", "lang": "en"}, {"value": "Potenzial für den abiotischen Abbau nicht fossiler Ressourcen (ADPE)", "lang": "de"}], "type": "LCIA method data set", "refObjectId": "b2ad6494-c78d-11e6-9d9d-cec0c932ce01", "uri": "../lciamethods/b2ad6494-c78d-11e6-9d9d-cec0c932ce01.xml"}, "other": {"anies": [{"name": "referenceToUnitGroupDataSet", "value": {"shortDescription": [{"value": "kg Sb-Äq.", "lang": "en"}], "type": "unit group data set", "refObjectId": "54ccd2d9-a32a-4fc2-923d-f2c8c93e89d4", "uri": "../unitgroups/54ccd2d9-a32a-4fc2-923d-f2c8c93e89d4.xml"}}, {"value": "5.23934E-07", "module": "A1-A3"}, {"value": "3.94383E-08", "module": "A4"}, {"value": "4.5893E-08", "module": "A5"}, {"value": "1.91E-07", "module": "B1"}, {"value": "4.43E-08", "module": "C1"}, {"value": "1.96682E-08", "module": "C2"}, {"value": "2.8181E-08", "module": "C3"}, {"value": "1.75E-07", "module": "C4"}, {"value": "-7.23E-08", "module": "D"}]}}, {"referenceToLCIAMethodDataSet": {"shortDescription": [{"value": "Abiotic depletion potential for fossil resources (ADPF)", "lang": "en"}, {"value": "Potenzial für den abiotischen Abbau fossiler Brennstoffe (ADPF)", "lang": "de"}], "type": "LCIA method data set", "refObjectId": "b2ad6110-c78d-11e6-9d9d-cec0c932ce01", "uri": "../lciamethods/b2ad6110-c78d-11e6-9d9d-cec0c932ce01.xml"}, "other": {"anies": [{"name": "referenceToUnitGroupDataSet", "value": {"shortDescription": [{"value": "MJ", "lang": "en"}], "type": "unit group data set", "refObjectId": "93a60a57-a3c8-11da-a746-0800200c9a66", "uri": "../unitgroups/93a60a57-a3c8-11da-a746-0800200c9a66.xml"}}, {"value": "47.3895", "module": "A1-A3"}, {"value": "6.30369", "module": "A4"}, {"value": "7.2384", "module": "A5"}, {"value": "2.04", "module": "B1"}, {"value": "7.08", "module": "C1"}, {"value": "3.14674", "module": "C2"}, {"value": "2.5618", "module": "C3"}, {"value": "29.1", "module": "C4"}, {"value": "-6.256", "module": "D"}]}}, {"referenceToLCIAMethodDataSet": {"shortDescription": [{"value": "Water use (WDP)", "lang": "en"}, {"value": "Wassernutzung (WDP)", "lang": "de"}], "type": "LCIA method data set", "refObjectId": "b2ad66ce-c78d-11e6-9d9d-cec0c932ce01", "uri": "../lciamethods/b2ad66ce-c78d-11e6-9d9d-cec0c932ce01.xml"}, "other": {"anies": [{"name": "referenceToUnitGroupDataSet", "value": {"shortDescription": [{"value": "m^(3) world-Äq. deprived", "lang": "en"}], "type": "unit group data set", "refObjectId": "6ae2df01-888e-46c8-b17d-49fa3869b476", "uri": "../unitgroups/6ae2df01-888e-46c8-b17d-49fa3869b476.xml"}}, {"value": "0.14432596", "module": "A1-A3"}, {"value": "0.00203922", "module": "A4"}, {"value": "0.0674", "module": "A5"}, {"value": "0.00317", "module": "B1"}, {"value": "0.0023", "module": "C1"}, {"value": "0.00102163", "module": "C2"}, {"value": "0.7088", "module": "C3"}, {"value": "0.171", "module": "C4"}, {"value": "-0.04906", "module": "D"}]}}, {"referenceToLCIAMethodDataSet": {"shortDescription": [{"value": "Incidence of disease due to PM emissions (PM)", "lang": "en"}, {"value": "Auftreten von Krankheiten aufgrund von Feinstaubemissionen (PM)", "lang": "de"}], "type": "LCIA method data set", "refObjectId": "b5c602c6-def3-11e6-bf01-fe55135034f3", "uri": "../lciamethods/b5c602c6-def3-11e6-bf01-fe55135034f3.xml"}, "other": {"anies": [{"name": "referenceToUnitGroupDataSet", "value": {"shortDescription": [{"value": "Disease incidence", "lang": "en"}], "type": "unit group data set", "refObjectId": "3883559b-648f-4afc-8ba2-0bd24f3affa3", "uri": "../unitgroups/3883559b-648f-4afc-8ba2-0bd24f3affa3.xml"}}, {"module": "A1-A3"}, {"module": "A4"}, {"module": "A5"}, {"module": "B1"}, {"module": "C1"}, {"module": "C2"}, {"module": "C3"}, {"module": "C4"}, {"module": "D"}]}}, {"referenceToLCIAMethodDataSet": {"shortDescription": [{"value": "Human exposure efficiency relative to U235 (IR)", "lang": "en"}, {"value": "Wirkung durch Exposition des Menschen mit U235 (IR)", "lang": "de"}], "type": "LCIA method data set", "refObjectId": "b5c632be-def3-11e6-bf01-fe55135034f3", "uri": "../lciamethods/b5c632be-def3-11e6-bf01-fe55135034f3.xml"}, "other": {"anies": [{"name": "referenceToUnitGroupDataSet", "value": {"shortDescription": [{"value": "kBq U235-Äq.", "lang": "en"}], "type": "unit group data set", "refObjectId": "456b05bf-1415-44a9-9993-02452f554c09", "uri": "../unitgroups/456b05bf-1415-44a9-9993-02452f554c09.xml"}}, {"module": "A1-A3"}, {"module": "A4"}, {"module": "A5"}, {"module": "B1"}, {"module": "C1"}, {"module": "C2"}, {"module": "C3"}, {"module": "C4"}, {"module": "D"}]}}, {"referenceToLCIAMethodDataSet": {"shortDescription": [{"value": "Comparative toxic unit for ecosystems (ETP-fw)", "lang": "en"}, {"value": "Toxizitätsvergleichseinheit für Ökosysteme (ETP-fw)", "lang": "de"}], "type": "LCIA method data set", "refObjectId": "ee1082d1-b0f7-43ca-a1f0-21e2a4a74511", "uri": "../lciamethods/ee1082d1-b0f7-43ca-a1f0-21e2a4a74511.xml"}, "other": {"anies": [{"name": "referenceToUnitGroupDataSet", "value": {"shortDescription": [{"value": "CTUe", "lang": "en"}], "type": "unit group data set", "refObjectId": "aa959ded-f1eb-4efb-9c5c-2d60be36b3e6", "uri": "../unitgroups/aa959ded-f1eb-4efb-9c5c-2d60be36b3e6.xml"}}, {"module": "A1-A3"}, {"module": "A4"}, {"module": "A5"}, {"module": "B1"}, {"module": "C1"}, {"module": "C2"}, {"module": "C3"}, {"module": "C4"}, {"module": "D"}]}}, {"referenceToLCIAMethodDataSet": {"shortDescription": [{"value": "Comparative toxic unit for humans (carcinogenic) (HTP-c)", "lang": "en"}, {"value": "Toxizitätsvergleichseinheit für Menschen (krebserregend) (HTP-c)", "lang": "de"}], "type": "LCIA method data set", "refObjectId": "2299222a-bbd8-474f-9d4f-4dd1f18aea7c", "uri": "../lciamethods/2299222a-bbd8-474f-9d4f-4dd1f18aea7c.xml"}, "other": {"anies": [{"name": "referenceToUnitGroupDataSet", "value": {"shortDescription": [{"value": "CTUh", "lang": "en"}], "type": "unit group data set", "refObjectId": "d4c9523e-2d7e-49fd-8469-998f547d3a70", "uri": "../unitgroups/d4c9523e-2d7e-49fd-8469-998f547d3a70.xml"}}, {"module": "A1-A3"}, {"module": "A4"}, {"module": "A5"}, {"module": "B1"}, {"module": "C1"}, {"module": "C2"}, {"module": "C3"}, {"module": "C4"}, {"module": "D"}]}}, {"referenceToLCIAMethodDataSet": {"shortDescription": [{"value": "Comparative toxic unit for humans (noncarcinogenic) (HTP-nc)", "lang": "en"}, {"value": "Toxizitätsvergleichseinheit für Menschen (nicht krebserregend) (HTP-nc)", "lang": "de"}], "type": "LCIA method data set", "refObjectId": "3af763a5-b7a1-48c9-9cee-1f223481fcef", "uri": "../lciamethods/3af763a5-b7a1-48c9-9cee-1f223481fcef.xml"}, "other": {"anies": [{"name": "referenceToUnitGroupDataSet", "value": {"shortDescription": [{"value": "CTUh", "lang": "en"}], "type": "unit group data set", "refObjectId": "d4c9523e-2d7e-49fd-8469-998f547d3a70", "uri": "../unitgroups/d4c9523e-2d7e-49fd-8469-998f547d3a70.xml"}}, {"module": "A1-A3"}, {"module": "A4"}, {"module": "A5"}, {"module": "B1"}, {"module": "C1"}, {"module": "C2"}, {"module": "C3"}, {"module": "C4"}, {"module": "D"}]}}, {"referenceToLCIAMethodDataSet": {"shortDescription": [{"value": "Soil quality index (SQP)", "lang": "en"}, {"value": "Bodenqualitätsindex (SQP)", "lang": "de"}], "type": "LCIA method data set", "refObjectId": "b2ad6890-c78d-11e6-9d9d-cec0c932ce01", "uri": "../lciamethods/b2ad6890-c78d-11e6-9d9d-cec0c932ce01.xml"}, "other": {"anies": [{"name": "referenceToUnitGroupDataSet", "value": {"shortDescription": [{"value": "SQP", "lang": "en"}], "type": "unit group data set", "refObjectId": "f130951c-e67f-4f7f-8dd4-665de3974e18", "uri": "../unitgroups/f130951c-e67f-4f7f-8dd4-665de3974e18.xml"}}, {"module": "A1-A3"}, {"module": "A4"}, {"module": "A5"}, {"module": "B1"}, {"module": "C1"}, {"module": "C2"}, {"module": "C3"}, {"module": "C4"}, {"module": "D"}]}}]}, "otherAttributes": {"{http://www.indata.network/EPD/2019}epd-version": "1.2"}, "version": "1.1", "locations": "../ILCDLocations.xml"}