{"processInformation": {"dataSetInformation": {"UUID": "1a7e73ef-4cd6-4e59-91e6-00e96e1957ce", "name": {"baseName": [{"value": "S Base foundation for temporary buildings and constructions (Solidum EST AS)", "lang": "en"}, {"value": "S Base Fundament für temporäre Gebäude und Konstruktionen (Solidum EST AS)", "lang": "de"}]}, "classificationInformation": {"classification": [{"class": [{"value": "Metalle", "level": 0, "classId": "4"}, {"value": "Stahl und Eisen", "level": 1, "classId": "4.1"}, {"value": "Stahlprofile", "level": 2, "classId": "4.1.03"}], "name": "OEKOBAU.DAT"}]}, "generalComment": [{"value": "The owner of this EPD shall be liable for the underlying information and evidence. The programme operator Kiwa-Ecobility Experts shall not be liable with respect to manufacturer data, life cycle assessment data and evidence.\r\nThis is a Cradle to gate with options EPD.\r\n", "lang": "en"}], "other": {"anies": [{"scenario": [{"description": [{"value": "- A payload factor of 50 percent was used for all truck transports, which in fact corresponds to a full delivery and empty return trip. A data set for a non-specific truck was used.; - Consumption of 0.043 MJ diesel per kilogram of the products is assumed for the demolition of end-of-life products.; - There are 2 End of life waste scenario for this LCA were determined.  Steel:  NMD ID 70, According to this standard, the waste treatment process comprises 94 % recycling, 5 % re-use and 1 % landfill.; PVC:  NMD ID 63, According to this standard, the waste treatment process comprises 80 % recycling, 10 % incineration and 10 % landfill.; - S Base production is primarily done at Schake GmbH's facility located at Volmarsteiner Straße 48, Hagen, which accounts for approximately 95% of the workload. The remaining 5%, specifically the powder coating process, is conducted at Eckeseyer Straße 195, Hagen. The distance between these two locations is 4 km,.  All calculations have been made based on Volmarsteiner Straße 48, Hagen, as the main production site.; - For the waste scenario, the closest profile to the actual geographical location should be selected. However, due to limited data, Rethink has proposed using EU and CH profiles.; - The Assembly stage (A5) is declared to account for the environmental impacts associated with the end-of-life of packaging. ", "lang": "en"}], "name": "Standard scenario", "default": true}]}, "<ns11:modules xmlns:ns11=\"http://openlca.org/epd_ilcd\" xmlns=\"http://lca.jrc.it/ILCD/Process\" xmlns:c=\"http://lca.jrc.it/ILCD/Contact\" xmlns:common=\"http://lca.jrc.it/ILCD/Common\" xmlns:epd=\"http://www.iai.kit.edu/EPD/2013\" xmlns:epd2=\"http://www.indata.network/EPD/2019\" xmlns:f=\"http://lca.jrc.it/ILCD/Flow\" xmlns:fp=\"http://lca.jrc.it/ILCD/FlowProperty\" xmlns:m=\"http://lca.jrc.it/ILCD/LCIAMethod\" xmlns:s=\"http://lca.jrc.it/ILCD/Source\" xmlns:u=\"http://lca.jrc.it/ILCD/UnitGroup\" name=\"A1\" scenario=\"Standard scenario\"/>", "<ns11:modules xmlns:ns11=\"http://openlca.org/epd_ilcd\" xmlns=\"http://lca.jrc.it/ILCD/Process\" xmlns:c=\"http://lca.jrc.it/ILCD/Contact\" xmlns:common=\"http://lca.jrc.it/ILCD/Common\" xmlns:epd=\"http://www.iai.kit.edu/EPD/2013\" xmlns:epd2=\"http://www.indata.network/EPD/2019\" xmlns:f=\"http://lca.jrc.it/ILCD/Flow\" xmlns:fp=\"http://lca.jrc.it/ILCD/FlowProperty\" xmlns:m=\"http://lca.jrc.it/ILCD/LCIAMethod\" xmlns:s=\"http://lca.jrc.it/ILCD/Source\" xmlns:u=\"http://lca.jrc.it/ILCD/UnitGroup\" name=\"A1-A3\" scenario=\"Standard scenario\"/>", "<ns11:modules xmlns:ns11=\"http://openlca.org/epd_ilcd\" xmlns=\"http://lca.jrc.it/ILCD/Process\" xmlns:c=\"http://lca.jrc.it/ILCD/Contact\" xmlns:common=\"http://lca.jrc.it/ILCD/Common\" xmlns:epd=\"http://www.iai.kit.edu/EPD/2013\" xmlns:epd2=\"http://www.indata.network/EPD/2019\" xmlns:f=\"http://lca.jrc.it/ILCD/Flow\" xmlns:fp=\"http://lca.jrc.it/ILCD/FlowProperty\" xmlns:m=\"http://lca.jrc.it/ILCD/LCIAMethod\" xmlns:s=\"http://lca.jrc.it/ILCD/Source\" xmlns:u=\"http://lca.jrc.it/ILCD/UnitGroup\" name=\"A2\" scenario=\"Standard scenario\"/>", "<ns11:modules xmlns:ns11=\"http://openlca.org/epd_ilcd\" xmlns=\"http://lca.jrc.it/ILCD/Process\" xmlns:c=\"http://lca.jrc.it/ILCD/Contact\" xmlns:common=\"http://lca.jrc.it/ILCD/Common\" xmlns:epd=\"http://www.iai.kit.edu/EPD/2013\" xmlns:epd2=\"http://www.indata.network/EPD/2019\" xmlns:f=\"http://lca.jrc.it/ILCD/Flow\" xmlns:fp=\"http://lca.jrc.it/ILCD/FlowProperty\" xmlns:m=\"http://lca.jrc.it/ILCD/LCIAMethod\" xmlns:s=\"http://lca.jrc.it/ILCD/Source\" xmlns:u=\"http://lca.jrc.it/ILCD/UnitGroup\" name=\"A3\" scenario=\"Standard scenario\"/>", "<ns11:modules xmlns:ns11=\"http://openlca.org/epd_ilcd\" xmlns=\"http://lca.jrc.it/ILCD/Process\" xmlns:c=\"http://lca.jrc.it/ILCD/Contact\" xmlns:common=\"http://lca.jrc.it/ILCD/Common\" xmlns:epd=\"http://www.iai.kit.edu/EPD/2013\" xmlns:epd2=\"http://www.indata.network/EPD/2019\" xmlns:f=\"http://lca.jrc.it/ILCD/Flow\" xmlns:fp=\"http://lca.jrc.it/ILCD/FlowProperty\" xmlns:m=\"http://lca.jrc.it/ILCD/LCIAMethod\" xmlns:s=\"http://lca.jrc.it/ILCD/Source\" xmlns:u=\"http://lca.jrc.it/ILCD/UnitGroup\" name=\"A5\" scenario=\"Standard scenario\"/>", "<ns11:modules xmlns:ns11=\"http://openlca.org/epd_ilcd\" xmlns=\"http://lca.jrc.it/ILCD/Process\" xmlns:c=\"http://lca.jrc.it/ILCD/Contact\" xmlns:common=\"http://lca.jrc.it/ILCD/Common\" xmlns:epd=\"http://www.iai.kit.edu/EPD/2013\" xmlns:epd2=\"http://www.indata.network/EPD/2019\" xmlns:f=\"http://lca.jrc.it/ILCD/Flow\" xmlns:fp=\"http://lca.jrc.it/ILCD/FlowProperty\" xmlns:m=\"http://lca.jrc.it/ILCD/LCIAMethod\" xmlns:s=\"http://lca.jrc.it/ILCD/Source\" xmlns:u=\"http://lca.jrc.it/ILCD/UnitGroup\" name=\"C1\" scenario=\"Standard scenario\"/>", "<ns11:modules xmlns:ns11=\"http://openlca.org/epd_ilcd\" xmlns=\"http://lca.jrc.it/ILCD/Process\" xmlns:c=\"http://lca.jrc.it/ILCD/Contact\" xmlns:common=\"http://lca.jrc.it/ILCD/Common\" xmlns:epd=\"http://www.iai.kit.edu/EPD/2013\" xmlns:epd2=\"http://www.indata.network/EPD/2019\" xmlns:f=\"http://lca.jrc.it/ILCD/Flow\" xmlns:fp=\"http://lca.jrc.it/ILCD/FlowProperty\" xmlns:m=\"http://lca.jrc.it/ILCD/LCIAMethod\" xmlns:s=\"http://lca.jrc.it/ILCD/Source\" xmlns:u=\"http://lca.jrc.it/ILCD/UnitGroup\" name=\"C2\" scenario=\"Standard scenario\"/>", "<ns11:modules xmlns:ns11=\"http://openlca.org/epd_ilcd\" xmlns=\"http://lca.jrc.it/ILCD/Process\" xmlns:c=\"http://lca.jrc.it/ILCD/Contact\" xmlns:common=\"http://lca.jrc.it/ILCD/Common\" xmlns:epd=\"http://www.iai.kit.edu/EPD/2013\" xmlns:epd2=\"http://www.indata.network/EPD/2019\" xmlns:f=\"http://lca.jrc.it/ILCD/Flow\" xmlns:fp=\"http://lca.jrc.it/ILCD/FlowProperty\" xmlns:m=\"http://lca.jrc.it/ILCD/LCIAMethod\" xmlns:s=\"http://lca.jrc.it/ILCD/Source\" xmlns:u=\"http://lca.jrc.it/ILCD/UnitGroup\" name=\"C3\" scenario=\"Standard scenario\"/>", "<ns11:modules xmlns:ns11=\"http://openlca.org/epd_ilcd\" xmlns=\"http://lca.jrc.it/ILCD/Process\" xmlns:c=\"http://lca.jrc.it/ILCD/Contact\" xmlns:common=\"http://lca.jrc.it/ILCD/Common\" xmlns:epd=\"http://www.iai.kit.edu/EPD/2013\" xmlns:epd2=\"http://www.indata.network/EPD/2019\" xmlns:f=\"http://lca.jrc.it/ILCD/Flow\" xmlns:fp=\"http://lca.jrc.it/ILCD/FlowProperty\" xmlns:m=\"http://lca.jrc.it/ILCD/LCIAMethod\" xmlns:s=\"http://lca.jrc.it/ILCD/Source\" xmlns:u=\"http://lca.jrc.it/ILCD/UnitGroup\" name=\"C4\" scenario=\"Standard scenario\"/>", "<ns11:modules xmlns:ns11=\"http://openlca.org/epd_ilcd\" xmlns=\"http://lca.jrc.it/ILCD/Process\" xmlns:c=\"http://lca.jrc.it/ILCD/Contact\" xmlns:common=\"http://lca.jrc.it/ILCD/Common\" xmlns:epd=\"http://www.iai.kit.edu/EPD/2013\" xmlns:epd2=\"http://www.indata.network/EPD/2019\" xmlns:f=\"http://lca.jrc.it/ILCD/Flow\" xmlns:fp=\"http://lca.jrc.it/ILCD/FlowProperty\" xmlns:m=\"http://lca.jrc.it/ILCD/LCIAMethod\" xmlns:s=\"http://lca.jrc.it/ILCD/Source\" xmlns:u=\"http://lca.jrc.it/ILCD/UnitGroup\" name=\"D\" scenario=\"Standard scenario\"/>"]}}, "quantitativeReference": {"referenceToReferenceFlow": [1], "type": "Reference flow(s)"}, "time": {"referenceYear": 2024, "dataSetValidUntil": 2030, "timeRepresentativenessDescription": [{"value": "All primary data were collected by manufacture of product  Schake GmbH  for the reference year of 2024 covering the period from January to December 2024.", "lang": "en"}], "other": {"anies": [{"name": "publicationDateOfEPD", "value": 1739923200000}]}}, "geography": {"locationOfOperationSupplyOrProduction": {"descriptionOfRestrictions": [{"value": "The results of this EPD are representative for European Union.", "lang": "en"}], "location": "EU-27"}}, "technology": {"technologyDescriptionAndIncludedProcesses": [{"value": "The S-Base™ is a foundation system developed by Solidum EST in Norway and is manufactured under license by Schake GmbH in Germany. Market for the product is EU and Nordic countries. The business model is based on rental or subscription solutions.  All components are equipped with unique serial numbers, ensuring traceability. Each foundation is fitted with QR codes and RFID technology connected to quality system, providing a comprehensive view of where the foundations are used and where they have been used throughout their entire lifecycle. \r\nIndividual components such as Steel (Steel S235 JR,Steel S235 JRH,Steel S355 J2H, Steel S235, Steel G3Si1), 360 PVC soft,  welding consumables, coating materials , and other ancillary materials are delivered to the production facility. All the raw materials are mainly delivered by truck. Until the materials are actually used in production, they are stored in the warehouse. The processes that are performed at the production facility are: cutting of profiles and plates, assembly, welding, sand blasting, priming and painting of structures (paint layer depends on customer’s requirements) and packing for a delivery. All inputs, including raw materials, primary products, energy, and auxiliary materials as well as the accumulated waste are considered in the assessment. \r\nProduction stage: There are two production locations for S Base. The primary production occurs at Schake GmbH's facility at Volmarsteiner Straße 48, Hagen, while the powder coating process is conducted at the second location at Eckeseyer Straße 195, Hagen. The manufacturing process for the S-Base™ foundation system begins with the selection of German steel (3-10 mm thick), recycled PVC base plates (360 PVC soft). Steel sheets and tubes are precision cut using CNC-controlled lasers for optimal resource efficiency. After cutting, components are assembled through a combination of manual and robotic welding to ensure strength and durability.\r\nPrior to coating, the steel undergoes multiple cleaning steps to enhance adhesion. The components are then hot-dip galvanized at 450 °C using renewable energy and finished with a green powder coating that meets C5 corrosion standards. The 360 PVC soft base plates are crafted from recycled materials. Final assembly utilizes stainless or acid-resistant fasteners, and each foundation is scanned via RFID for quality control before packaging.\r\n", "lang": "en"}], "technologicalApplicability": [{"value": "S Base is developed especially for temporary buildings  such as living quarters, porta cabins, canteens, office buildings, preschools or school buildings. There is also a special application to be used under steel containers.  After 6-180 months of use, the S Bases will be removed by crane truck, sent to a local hub for inspection and maintenance and then reused for the next project.", "lang": "en"}], "referenceToTechnologyFlowDiagrammOrPicture": [{"shortDescription": [{"value": "Flow chart S Base foundation for temporary buildings and constructions (Solidum EST AS)", "lang": "en"}], "type": "source data set", "refObjectId": "eeb2a55a-6624-4360-9851-8292b7f464c9", "version": "00.00.001"}]}}, "modellingAndValidation": {"LCIMethodAndAllocation": {"typeOfDataSet": "EPD", "other": {"anies": [{"name": "subType", "value": "specific dataset"}]}}, "dataSourcesTreatmentAndRepresentativeness": {"referenceToDataSource": [{"shortDescription": [{"value": "ecoinvent 3.6 database", "lang": "en"}], "type": "source data set", "refObjectId": "766b9973-5ee8-48a2-8098-72c8e20b369f", "version": "00.00.001"}, {"shortDescription": [{"value": "ecoinvent database (general)", "lang": "en"}], "type": "source data set", "refObjectId": "b497a91f-e14b-4b69-8f28-f50eb1576766", "version": "00.03.002"}], "useAdviceForDataSet": [{"value": "S Base is developed especially for temporary buildings  such as living quarters, porta cabins, canteens, office buildings, preschools or school buildings. There is also a special application to be used under steel containers.  After 6-180 months of use, the S Bases will be removed by crane truck, sent to a local hub for inspection and maintenance and then reused for the next project.", "lang": "en"}], "other": {"anies": [{"name": "referenceToOriginalEPD", "value": {"shortDescription": {"value": "S Base foundation for temporary buildings and constructions (Solidum EST AS) EPD", "defaultValue": "S Base foundation for temporary buildings and constructions (Solidum EST AS) EPD", "lstrings": [{"lang": "en", "value": "S Base foundation for temporary buildings and constructions (Solidum EST AS) EPD"}]}, "version": {"version": 2, "majorVersion": 0, "minorVersion": 0, "subMinorVersion": 2, "zero": false, "versionString": "00.00.002"}, "type": "source data set", "uuid": {"uuid": "9ad1648e-f7f8-49fd-8259-eb971fd4e0b2"}, "refObjectId": "9ad1648e-f7f8-49fd-8259-eb971fd4e0b2", "versionAsString": "00.00.002", "resourceURLs": ["https://oekobaudat.de/OEKOBAU.DAT/resource/sources/9ad1648e-f7f8-49fd-8259-eb971fd4e0b2/91318-s-base-foundation-for-temporary-buildings-and-constructions--202502191013-long.pdf?version=00.00.002"]}}]}}, "validation": {"review": [{"reviewDetails": [{"value": "The independent verification is in accordance with the ISO 14025:2011. ", "lang": "en"}], "referenceToNameOfReviewerAndInstitution": [{"shortDescription": [{"value": "Kripanshi Gupta, Kiwa GmbH", "lang": "en"}], "type": "contact data set", "refObjectId": "0b3c94ec-437c-4241-8479-572039fe43bb", "version": "00.00.001"}], "type": "Independent external review"}]}, "complianceDeclarations": {"compliance": [{"referenceToComplianceSystem": {"shortDescription": [{"value": "ISO 14025", "lang": "en"}], "type": "source data set", "refObjectId": "4f2eb655-6e44-4874-a95a-e28f5442cd4d", "version": "00.00.001"}}, {"referenceToComplianceSystem": {"shortDescription": [{"value": "EN 15804+A2 (EF 3.1)", "lang": "de"}, {"value": "EN 15804+A2 (EF 3.1)", "lang": "en"}], "type": "source data set", "refObjectId": "d4aa3ec7-b1d7-4a4a-a6cb-37af88dcc902", "version": "00.01.000"}}]}}, "administrativeInformation": {"commissionerAndGoal": {"referenceToCommissioner": [{"shortDescription": [{"value": "Solidum EST AS", "lang": "en"}], "type": "contact data set", "refObjectId": "6f796b5b-10dd-4e8a-8e34-58bcd77070a0", "version": "00.00.001"}]}, "dataGenerator": {"referenceToPersonOrEntityGeneratingTheDataSet": [{"shortDescription": [{"value": "Kiwa Kompetanse AS ", "lang": "en"}], "type": "contact data set", "refObjectId": "5dd98ed3-fefd-48c7-b3b7-cc7e57d9d7c5", "version": "00.00.001"}]}, "dataEntryBy": {"timeStamp": 1745320728627, "referenceToDataSetFormat": [{"shortDescription": [{"value": "EPD Data Format Extensions v1.2", "lang": "en"}, {"value": "EPD-Datenformaterweiterungen v1.2", "lang": "de"}], "type": "source data set", "refObjectId": "a29449fd-aa2f-4de8-b5d7-4b06b43c6fde", "version": "00.01.000"}, {"shortDescription": [{"value": "ILCD format", "lang": "en"}], "type": "source data set", "refObjectId": "a97a0155-0234-4b87-b4ce-a45da52f2a40", "version": "01.00.000", "uri": "http://lca.jrc.ec.europa.eu/lcainfohub/sample_data/ilcd/sources/ILCD_Format_a97a0155-0234-4b87-b4ce-a45da52f2a40_01.00.000.xml"}], "referenceToPersonOrEntityEnteringTheData": {"shortDescription": [{"value": "Kiwa-Ecobility Experts, Kiwa GmbH (Berlin)", "lang": "en"}], "type": "contact data set", "refObjectId": "eb52a9a8-9d0f-40ce-a5c9-7b78f5615e5a", "version": "00.00.002"}}, "publicationAndOwnership": {"dataSetVersion": "00.00.013", "referenceToRegistrationAuthority": {"shortDescription": [{"value": "Kiwa-Ecobility Experts, Kiwa GmbH (Berlin)", "lang": "en"}], "type": "contact data set", "refObjectId": "eb52a9a8-9d0f-40ce-a5c9-7b78f5615e5a", "version": "00.00.002"}, "registrationNumber": "EPD-Kiwa-EE-191318-EN", "referenceToOwnershipOfDataSet": {"shortDescription": [{"value": "Solidum EST AS", "lang": "en"}], "type": "contact data set", "refObjectId": "6f796b5b-10dd-4e8a-8e34-58bcd77070a0", "version": "00.00.001"}, "copyright": true, "licenseType": "Free of charge for all users and uses", "accessRestrictions": [{"value": "None.", "lang": "en"}], "other": {"anies": [{"name": "referenceToPublisher", "value": {"shortDescription": [{"value": "Kiwa-Ecobility Experts, Kiwa GmbH (Berlin)", "lang": "en"}], "type": "contact data set", "refObjectId": "eb52a9a8-9d0f-40ce-a5c9-7b78f5615e5a", "version": "00.00.002"}}]}}}, "exchanges": {"exchange": [{"dataSetInternalID": 1, "referenceToFlowDataSet": {"shortDescription": [{"value": "S Base foundation for temporary buildings and constructions (Solidum EST AS)", "lang": "en"}, {"value": "S Base Fundament für temporäre Gebäude und Konstruktionen (Solidum EST AS)", "lang": "de"}], "type": "flow data set", "refObjectId": "5679fac4-5259-4bc1-9edb-cb0f15c1c6a4", "version": "00.00.003"}, "meanAmount": 1.0, "resultingAmount": 1.0, "referenceFlow": true, "resultingflowAmount": 1.0, "flowProperties": [{"name": [{"lang": "de", "value": "Anzahl"}, {"lang": "en", "value": "Number of pieces"}], "uuid": "01846770-4cfe-4a25-8ad9-919d8d378345", "referenceFlowProperty": true, "meanValue": 1.0, "referenceUnit": "pcs.", "unitGroupUUID": "934110e3-baf4-49e9-992c-3d8109a6aafb"}], "materialProperties": [{"name": "weight per piece", "value": "37.445", "unit": "kg"}], "typeOfFlow": "Product flow", "classification": {"classHierarchy": "Metalle / Stahl und Eisen / Stahlprofile", "name": "OEKOBAU.DAT"}}, {"dataSetInternalID": 2, "referenceToFlowDataSet": {"shortDescription": [{"value": "Components for re-use (CRU)", "lang": "en"}, {"value": "Komponenten für die Wiederverwendung (CRU)", "lang": "de"}, {"value": "Componentes para su reutilización (CRU)", "lang": "es"}], "type": "flow data set", "refObjectId": "a2b32f97-3fc7-4af2-b209-525bc6426f33", "version": "30.00.000", "uri": "../flows/a2b32f97-3fc7-4af2-b209-525bc6426f33.xml"}, "exchange direction": "OUTPUT", "meanAmount": 0.0, "other": {"anies": [{"value": "0.0", "module": "A1", "scenario": "Standard scenario"}, {"value": "0.0", "module": "A2", "scenario": "Standard scenario"}, {"value": "5.71E-5", "module": "A3", "scenario": "Standard scenario"}, {"value": "5.71E-5", "module": "A1-A3", "scenario": "Standard scenario"}, {"value": "0.005", "module": "A5", "scenario": "Standard scenario"}, {"value": "0.0", "module": "C1", "scenario": "Standard scenario"}, {"value": "0.0", "module": "C2", "scenario": "Standard scenario"}, {"value": "0.571", "module": "C3", "scenario": "Standard scenario"}, {"value": "0.0", "module": "C4", "scenario": "Standard scenario"}, {"value": "0.0", "module": "D", "scenario": "Standard scenario"}, {"name": "referenceToUnitGroupDataSet", "value": {"shortDescription": [{"value": "kg", "lang": "en"}], "type": "unit group data set", "refObjectId": "ad38d542-3fe9-439d-9b95-2f5f7752acaf", "version": "30.00.000", "uri": "../unitgroups/ad38d542-3fe9-439d-9b95-2f5f7752acaf.xml"}}]}, "flowProperties": [], "typeOfFlow": "Other flow", "classification": {"classHierarchy": "Größen / Umweltliche Größen / EPD EN 15804 / LCI Indikatoren", "name": "GaBiCategories"}}, {"dataSetInternalID": 3, "referenceToFlowDataSet": {"shortDescription": [{"value": "Exported electrical energy (EEE)", "lang": "en"}, {"value": "Exportierte elektrische Energie (EEE)", "lang": "de"}, {"value": "Energía exportada electrica (EEE)", "lang": "es"}], "type": "flow data set", "refObjectId": "4da0c987-2b76-40d6-9e9e-82a017aaaf29", "version": "30.00.000", "uri": "../flows/4da0c987-2b76-40d6-9e9e-82a017aaaf29.xml"}, "exchange direction": "OUTPUT", "meanAmount": 0.0, "other": {"anies": [{"value": "0.0", "module": "A1", "scenario": "Standard scenario"}, {"value": "0.0", "module": "A2", "scenario": "Standard scenario"}, {"value": "-1.1777175E-5", "module": "A3", "scenario": "Standard scenario"}, {"value": "-1.1777175E-5", "module": "A1-A3", "scenario": "Standard scenario"}, {"value": "0.0", "module": "A5", "scenario": "Standard scenario"}, {"value": "0.0", "module": "C1", "scenario": "Standard scenario"}, {"value": "0.0", "module": "C2", "scenario": "Standard scenario"}, {"value": "0.0", "module": "C3", "scenario": "Standard scenario"}, {"value": "0.0", "module": "C4", "scenario": "Standard scenario"}, {"value": "-6.00406425", "module": "D", "scenario": "Standard scenario"}, {"name": "referenceToUnitGroupDataSet", "value": {"shortDescription": [{"value": "MJ", "lang": "en"}], "type": "unit group data set", "refObjectId": "93a60a57-a3c8-11da-a746-0800200c9a66", "version": "03.00.000", "uri": "../unitgroups/93a60a57-a3c8-11da-a746-0800200c9a66.xml"}}]}, "flowProperties": [], "typeOfFlow": "Other flow", "classification": {"classHierarchy": "Größen / Umweltliche Größen / EPD EN 15804 / LCI Indikatoren", "name": "GaBiCategories"}}, {"dataSetInternalID": 4, "referenceToFlowDataSet": {"shortDescription": [{"value": "Exported thermal energy (EET)", "lang": "en"}, {"value": "Exportierte thermische Energie (EET)", "lang": "de"}, {"value": "Energía exportada termal (EET)", "lang": "es"}], "type": "flow data set", "refObjectId": "98daf38a-7a79-46d3-9a37-2b7bd0955810", "version": "30.00.000", "uri": "../flows/98daf38a-7a79-46d3-9a37-2b7bd0955810.xml"}, "exchange direction": "OUTPUT", "meanAmount": 0.0, "other": {"anies": [{"value": "0.0", "module": "A1", "scenario": "Standard scenario"}, {"value": "0.0", "module": "A2", "scenario": "Standard scenario"}, {"value": "-2.02829125E-5", "module": "A3", "scenario": "Standard scenario"}, {"value": "-2.02829125E-5", "module": "A1-A3", "scenario": "Standard scenario"}, {"value": "0.0", "module": "A5", "scenario": "Standard scenario"}, {"value": "0.0", "module": "C1", "scenario": "Standard scenario"}, {"value": "0.0", "module": "C2", "scenario": "Standard scenario"}, {"value": "0.0", "module": "C3", "scenario": "Standard scenario"}, {"value": "0.0", "module": "C4", "scenario": "Standard scenario"}, {"value": "-10.340332875", "module": "D", "scenario": "Standard scenario"}, {"name": "referenceToUnitGroupDataSet", "value": {"shortDescription": [{"value": "MJ", "lang": "en"}], "type": "unit group data set", "refObjectId": "93a60a57-a3c8-11da-a746-0800200c9a66", "version": "03.00.000", "uri": "../unitgroups/93a60a57-a3c8-11da-a746-0800200c9a66.xml"}}]}, "flowProperties": [], "typeOfFlow": "Other flow", "classification": {"classHierarchy": "Größen / Umweltliche Größen / EPD EN 15804 / LCI Indikatoren", "name": "GaBiCategories"}}, {"dataSetInternalID": 5, "referenceToFlowDataSet": {"shortDescription": [{"value": "Use of net fresh water (FW)", "lang": "en"}, {"value": "Einsatz von Süßwasserressourcen (FW)", "lang": "de"}, {"value": "Uso neto de recursos de agua dulce (FW)", "lang": "es"}], "type": "flow data set", "refObjectId": "3cf952c8-f3a4-461d-8c96-96456ca62246", "version": "30.00.000", "uri": "../flows/3cf952c8-f3a4-461d-8c96-96456ca62246.xml"}, "exchange direction": "INPUT", "meanAmount": 0.0, "other": {"anies": [{"value": "0.29503556633871", "module": "A1", "scenario": "Standard scenario"}, {"value": "0.00121051773305", "module": "A2", "scenario": "Standard scenario"}, {"value": "0.01546819198639", "module": "A3", "scenario": "Standard scenario"}, {"value": "0.31171427605814994", "module": "A1-A3", "scenario": "Standard scenario"}, {"value": "0.00132962566854", "module": "A5", "scenario": "Standard scenario"}, {"value": "9.551121096E-5", "module": "C1", "scenario": "Standard scenario"}, {"value": "5.5577795285E-4", "module": "C2", "scenario": "Standard scenario"}, {"value": "0.08414034625", "module": "C3", "scenario": "Standard scenario"}, {"value": "6.971844E-4", "module": "C4", "scenario": "Standard scenario"}, {"value": "-0.04792560282397", "module": "D", "scenario": "Standard scenario"}, {"name": "referenceToUnitGroupDataSet", "value": {"shortDescription": [{"value": "m3", "lang": "en"}], "type": "unit group data set", "refObjectId": "cd950537-0a98-4044-9ba7-9f9a68d0a504", "version": "30.00.000", "uri": "../unitgroups/cd950537-0a98-4044-9ba7-9f9a68d0a504.xml"}}]}, "flowProperties": [], "typeOfFlow": "Other flow", "classification": {"classHierarchy": "Größen / Umweltliche Größen / EPD EN 15804 / LCI Indikatoren", "name": "GaBiCategories"}}, {"dataSetInternalID": 6, "referenceToFlowDataSet": {"shortDescription": [{"value": "Hazardous waste disposed (HWD)", "lang": "en"}, {"value": "Gefährlicher Abfall zur Deponie (HWD)", "lang": "de"}, {"value": "Residuos peligrosos eliminados (HWD)", "lang": "es"}], "type": "flow data set", "refObjectId": "430f9e0f-59b2-46a0-8e0d-55e0e84948fc", "version": "30.00.000", "uri": "../flows/430f9e0f-59b2-46a0-8e0d-55e0e84948fc.xml"}, "exchange direction": "OUTPUT", "meanAmount": 0.0, "other": {"anies": [{"value": "0.00242884476071", "module": "A1", "scenario": "Standard scenario"}, {"value": "2.518278408E-5", "module": "A2", "scenario": "Standard scenario"}, {"value": "7.283065465E-5", "module": "A3", "scenario": "Standard scenario"}, {"value": "0.00252685819944", "module": "A1-A3", "scenario": "Standard scenario"}, {"value": "2.67884137E-6", "module": "A5", "scenario": "Standard scenario"}, {"value": "5.05299232E-6", "module": "C1", "scenario": "Standard scenario"}, {"value": "1.156202491E-5", "module": "C2", "scenario": "Standard scenario"}, {"value": "1.548350375E-4", "module": "C3", "scenario": "Standard scenario"}, {"value": "1.0166765E-6", "module": "C4", "scenario": "Standard scenario"}, {"value": "-0.00160722280951", "module": "D", "scenario": "Standard scenario"}, {"name": "referenceToUnitGroupDataSet", "value": {"shortDescription": [{"value": "kg", "lang": "en"}], "type": "unit group data set", "refObjectId": "ad38d542-3fe9-439d-9b95-2f5f7752acaf", "version": "30.00.000", "uri": "../unitgroups/ad38d542-3fe9-439d-9b95-2f5f7752acaf.xml"}}]}, "flowProperties": [], "typeOfFlow": "Other flow", "classification": {"classHierarchy": "Größen / Umweltliche Größen / EPD EN 15804 / LCI Indikatoren", "name": "GaBiCategories"}}, {"dataSetInternalID": 7, "referenceToFlowDataSet": {"shortDescription": [{"value": "Materials for energy recovery (MER)", "lang": "en"}, {"value": "Stoffe für die Energierückgewinnung (MER)", "lang": "de"}, {"value": "Materiales para valorización energética (recuperación de energía) (MER)", "lang": "es"}], "type": "flow data set", "refObjectId": "59a9181c-3aaf-46ee-8b13-2b3723b6e447", "version": "30.00.000", "uri": "../flows/59a9181c-3aaf-46ee-8b13-2b3723b6e447.xml"}, "exchange direction": "OUTPUT", "meanAmount": 0.0, "other": {"anies": [{"value": "0.0", "module": "A1", "scenario": "Standard scenario"}, {"value": "0.0", "module": "A2", "scenario": "Standard scenario"}, {"value": "0.0", "module": "A3", "scenario": "Standard scenario"}, {"value": "0.0", "module": "A1-A3", "scenario": "Standard scenario"}, {"value": "0.0", "module": "A5", "scenario": "Standard scenario"}, {"value": "0.0", "module": "C1", "scenario": "Standard scenario"}, {"value": "0.0", "module": "C2", "scenario": "Standard scenario"}, {"value": "0.0", "module": "C3", "scenario": "Standard scenario"}, {"value": "0.0", "module": "C4", "scenario": "Standard scenario"}, {"value": "0.0", "module": "D", "scenario": "Standard scenario"}, {"name": "referenceToUnitGroupDataSet", "value": {"shortDescription": [{"value": "kg", "lang": "en"}], "type": "unit group data set", "refObjectId": "ad38d542-3fe9-439d-9b95-2f5f7752acaf", "version": "30.00.000", "uri": "../unitgroups/ad38d542-3fe9-439d-9b95-2f5f7752acaf.xml"}}]}, "flowProperties": [], "typeOfFlow": "Other flow", "classification": {"classHierarchy": "Größen / Umweltliche Größen / EPD EN 15804 / LCI Indikatoren", "name": "GaBiCategories"}}, {"dataSetInternalID": 8, "referenceToFlowDataSet": {"shortDescription": [{"value": "Materials for recycling (MFR)", "lang": "en"}, {"value": "Stoffe zum Recycling (MFR)", "lang": "de"}, {"value": "Materiales para el reciclaje (MFR)", "lang": "es"}], "type": "flow data set", "refObjectId": "d7fe48a5-4103-49c8-9aae-b0b5dfdbd6ae", "version": "30.00.000", "uri": "../flows/d7fe48a5-4103-49c8-9aae-b0b5dfdbd6ae.xml"}, "exchange direction": "OUTPUT", "meanAmount": 0.0, "other": {"anies": [{"value": "0.0", "module": "A1", "scenario": "Standard scenario"}, {"value": "0.0", "module": "A2", "scenario": "Standard scenario"}, {"value": "0.003153605", "module": "A3", "scenario": "Standard scenario"}, {"value": "0.003153605", "module": "A1-A3", "scenario": "Standard scenario"}, {"value": "0.2315", "module": "A5", "scenario": "Standard scenario"}, {"value": "0.0", "module": "C1", "scenario": "Standard scenario"}, {"value": "0.0", "module": "C2", "scenario": "Standard scenario"}, {"value": "31.53605", "module": "C3", "scenario": "Standard scenario"}, {"value": "0.0", "module": "C4", "scenario": "Standard scenario"}, {"value": "0.0", "module": "D", "scenario": "Standard scenario"}, {"name": "referenceToUnitGroupDataSet", "value": {"shortDescription": [{"value": "kg", "lang": "en"}], "type": "unit group data set", "refObjectId": "ad38d542-3fe9-439d-9b95-2f5f7752acaf", "version": "30.00.000", "uri": "../unitgroups/ad38d542-3fe9-439d-9b95-2f5f7752acaf.xml"}}]}, "flowProperties": [], "typeOfFlow": "Other flow", "classification": {"classHierarchy": "Größen / Umweltliche Größen / EPD EN 15804 / LCI Indikatoren", "name": "GaBiCategories"}}, {"dataSetInternalID": 9, "referenceToFlowDataSet": {"shortDescription": [{"value": "Non-hazardous waste disposed (NHWD)", "lang": "en"}, {"value": "Entsorgter nicht gefährlicher Abfall (NHWD)", "lang": "de"}, {"value": "Residuos no peligrosos eliminados (NHWD)", "lang": "es"}], "type": "flow data set", "refObjectId": "b29ef66b-e286-4afa-949f-62f1a7b4d7fa", "version": "30.00.000", "uri": "../flows/b29ef66b-e286-4afa-949f-62f1a7b4d7fa.xml"}, "exchange direction": "OUTPUT", "meanAmount": 0.0, "other": {"anies": [{"value": "7.32510768722142", "module": "A1", "scenario": "Standard scenario"}, {"value": "0.63037540795189", "module": "A2", "scenario": "Standard scenario"}, {"value": "0.35145679108767", "module": "A3", "scenario": "Standard scenario"}, {"value": "8.306939886260981", "module": "A1-A3", "scenario": "Standard scenario"}, {"value": "0.34238716204814", "module": "A5", "scenario": "Standard scenario"}, {"value": "0.00219649666278", "module": "C1", "scenario": "Standard scenario"}, {"value": "0.28942058773315", "module": "C2", "scenario": "Standard scenario"}, {"value": "3.99218086", "module": "C3", "scenario": "Standard scenario"}, {"value": "2.7229372115", "module": "C4", "scenario": "Standard scenario"}, {"value": "-1.3365570261086", "module": "D", "scenario": "Standard scenario"}, {"name": "referenceToUnitGroupDataSet", "value": {"shortDescription": [{"value": "kg", "lang": "en"}], "type": "unit group data set", "refObjectId": "ad38d542-3fe9-439d-9b95-2f5f7752acaf", "version": "30.00.000", "uri": "../unitgroups/ad38d542-3fe9-439d-9b95-2f5f7752acaf.xml"}}]}, "flowProperties": [], "typeOfFlow": "Other flow", "classification": {"classHierarchy": "Größen / Umweltliche Größen / EPD EN 15804 / LCI Indikatoren", "name": "GaBiCategories"}}, {"dataSetInternalID": 10, "referenceToFlowDataSet": {"shortDescription": [{"value": "Use of non renewable secondary fuels (NRSF)", "lang": "en"}, {"value": "Nicht erneuerbare Sekundärbrennstoffe (NRSF)", "lang": "de"}, {"value": "Uso de combustibles secundarios no renovables (NRSF)", "lang": "es"}], "type": "flow data set", "refObjectId": "89def144-d39a-4287-b86f-efde453ddcb2", "version": "30.00.000", "uri": "../flows/89def144-d39a-4287-b86f-efde453ddcb2.xml"}, "exchange direction": "INPUT", "meanAmount": 0.0, "other": {"anies": [{"value": "0.0", "module": "A1", "scenario": "Standard scenario"}, {"value": "0.0", "module": "A2", "scenario": "Standard scenario"}, {"value": "0.0", "module": "A3", "scenario": "Standard scenario"}, {"value": "0.0", "module": "A1-A3", "scenario": "Standard scenario"}, {"value": "0.0", "module": "A5", "scenario": "Standard scenario"}, {"value": "0.0", "module": "C1", "scenario": "Standard scenario"}, {"value": "0.0", "module": "C2", "scenario": "Standard scenario"}, {"value": "0.0", "module": "C3", "scenario": "Standard scenario"}, {"value": "0.0", "module": "C4", "scenario": "Standard scenario"}, {"value": "0.0", "module": "D", "scenario": "Standard scenario"}, {"name": "referenceToUnitGroupDataSet", "value": {"shortDescription": [{"value": "MJ", "lang": "en"}], "type": "unit group data set", "refObjectId": "93a60a57-a3c8-11da-a746-0800200c9a66", "version": "03.00.000", "uri": "../unitgroups/93a60a57-a3c8-11da-a746-0800200c9a66.xml"}}]}, "flowProperties": [], "typeOfFlow": "Other flow", "classification": {"classHierarchy": "Größen / Umweltliche Größen / EPD EN 15804 / LCI Indikatoren", "name": "GaBiCategories"}}, {"dataSetInternalID": 11, "referenceToFlowDataSet": {"shortDescription": [{"value": "Use of non renewable primary energy (PENRE)", "lang": "en"}, {"value": "Nicht-erneuerbare Primärenergie als Energieträger (PENRE)", "lang": "de"}, {"value": "Uso de energía primaria no renovable, excluyendo los recursos de energía primaria no renovable utilizada como materia prima (PENRE)", "lang": "es"}], "type": "flow data set", "refObjectId": "ac857178-2b45-46ec-892a-a9a4332f0372", "version": "38.00.000", "uri": "../flows/ac857178-2b45-46ec-892a-a9a4332f0372.xml"}, "exchange direction": "INPUT", "meanAmount": 0.0, "other": {"anies": [{"value": "502.295503353621", "module": "A1", "scenario": "Standard scenario"}, {"value": "10.5510423688927", "module": "A2", "scenario": "Standard scenario"}, {"value": "31.0397186633867", "module": "A3", "scenario": "Standard scenario"}, {"value": "543.8862643859004", "module": "A1-A3", "scenario": "Standard scenario"}, {"value": "1.1721275728766", "module": "A5", "scenario": "Standard scenario"}, {"value": "1.9701448550422", "module": "C1", "scenario": "Standard scenario"}, {"value": "4.84423859985876", "module": "C2", "scenario": "Standard scenario"}, {"value": "103.3534186875", "module": "C3", "scenario": "Standard scenario"}, {"value": "0.7091969292", "module": "C4", "scenario": "Standard scenario"}, {"value": "-102.729192957847", "module": "D", "scenario": "Standard scenario"}, {"name": "referenceToUnitGroupDataSet", "value": {"shortDescription": [{"value": "MJ", "lang": "en"}], "type": "unit group data set", "refObjectId": "93a60a57-a3c8-11da-a746-0800200c9a66", "version": "03.00.000", "uri": "../unitgroups/93a60a57-a3c8-11da-a746-0800200c9a66.xml"}}]}, "flowProperties": [], "typeOfFlow": "Other flow", "classification": {"classHierarchy": "Quantities", "name": "GaBiCategories"}}, {"dataSetInternalID": 12, "referenceToFlowDataSet": {"shortDescription": [{"value": "Use of non renewable primary energy resources used as raw materials (PENRM)", "lang": "en"}, {"value": "Nicht-erneuerbare Primärenergie zur stofflichen Nutzung (PENRM)", "lang": "de"}, {"value": "Uso de la energía primaria no renovable utilizada como materia prima (PENRM)", "lang": "es"}], "type": "flow data set", "refObjectId": "1421caa0-679d-4bf4-b282-0eb850ccae27", "version": "38.00.000", "uri": "../flows/1421caa0-679d-4bf4-b282-0eb850ccae27.xml"}, "exchange direction": "INPUT", "meanAmount": 0.0, "other": {"anies": [{"value": "0.76975", "module": "A1", "scenario": "Standard scenario"}, {"value": "0.0", "module": "A2", "scenario": "Standard scenario"}, {"value": "7.34181375E-5", "module": "A3", "scenario": "Standard scenario"}, {"value": "0.7698234181375", "module": "A1-A3", "scenario": "Standard scenario"}, {"value": "0.0", "module": "A5", "scenario": "Standard scenario"}, {"value": "0.0", "module": "C1", "scenario": "Standard scenario"}, {"value": "0.0", "module": "C2", "scenario": "Standard scenario"}, {"value": "0.0", "module": "C3", "scenario": "Standard scenario"}, {"value": "0.0", "module": "C4", "scenario": "Standard scenario"}, {"value": "-0.035568625", "module": "D", "scenario": "Standard scenario"}, {"name": "referenceToUnitGroupDataSet", "value": {"shortDescription": [{"value": "MJ", "lang": "en"}], "type": "unit group data set", "refObjectId": "93a60a57-a3c8-11da-a746-0800200c9a66", "version": "03.00.000", "uri": "../unitgroups/93a60a57-a3c8-11da-a746-0800200c9a66.xml"}}]}, "flowProperties": [], "typeOfFlow": "Other flow", "classification": {"classHierarchy": "Quantities", "name": "GaBiCategories"}}, {"dataSetInternalID": 13, "referenceToFlowDataSet": {"shortDescription": [{"value": "Total use of non-renewable primary energy resources (PENRT)", "lang": "en"}, {"value": "Total nicht erneuerbare Primärenergie (PENRT)", "lang": "de"}, {"value": "Uso total de la energía primaria no renovable (energía primaria y recursos de energía primaria renovable utilizada como materia prima) (PENRT)", "lang": "es"}], "type": "flow data set", "refObjectId": "06159210-646b-4c8d-8583-da9b3b95a6c1", "version": "30.00.000", "uri": "../flows/06159210-646b-4c8d-8583-da9b3b95a6c1.xml"}, "exchange direction": "INPUT", "meanAmount": 0.0, "other": {"anies": [{"value": "503.065253353621", "module": "A1", "scenario": "Standard scenario"}, {"value": "10.5510423688927", "module": "A2", "scenario": "Standard scenario"}, {"value": "31.0397920815242", "module": "A3", "scenario": "Standard scenario"}, {"value": "544.656087804038", "module": "A1-A3", "scenario": "Standard scenario"}, {"value": "1.1721275728766", "module": "A5", "scenario": "Standard scenario"}, {"value": "1.9701448550422", "module": "C1", "scenario": "Standard scenario"}, {"value": "4.84423859985876", "module": "C2", "scenario": "Standard scenario"}, {"value": "103.3534186875", "module": "C3", "scenario": "Standard scenario"}, {"value": "0.7091969292", "module": "C4", "scenario": "Standard scenario"}, {"value": "-102.764761582847", "module": "D", "scenario": "Standard scenario"}, {"name": "referenceToUnitGroupDataSet", "value": {"shortDescription": [{"value": "MJ", "lang": "en"}], "type": "unit group data set", "refObjectId": "93a60a57-a3c8-11da-a746-0800200c9a66", "version": "03.00.000", "uri": "../unitgroups/93a60a57-a3c8-11da-a746-0800200c9a66.xml"}}]}, "flowProperties": [], "typeOfFlow": "Other flow", "classification": {"classHierarchy": "Größen / Umweltliche Größen / EPD EN 15804 / LCI Indikatoren", "name": "GaBiCategories"}}, {"dataSetInternalID": 14, "referenceToFlowDataSet": {"shortDescription": [{"value": "Use of renewable primary energy (PERE)", "lang": "en"}, {"value": "Erneuerbare Primärenergie als Energieträger (PERE)", "lang": "de"}, {"value": "Uso de energía primaria renovable excluyendo los recursos de energía primaria renovable utilizada como materia prima (PERE)", "lang": "es"}], "type": "flow data set", "refObjectId": "20f32be5-0398-4288-9b6d-accddd195317", "version": "38.00.000", "uri": "../flows/20f32be5-0398-4288-9b6d-accddd195317.xml"}, "exchange direction": "INPUT", "meanAmount": 0.0, "other": {"anies": [{"value": "40.3988699534339", "module": "A1", "scenario": "Standard scenario"}, {"value": "0.12441228200141", "module": "A2", "scenario": "Standard scenario"}, {"value": "43.2313738226156", "module": "A3", "scenario": "Standard scenario"}, {"value": "83.75465605805091", "module": "A1-A3", "scenario": "Standard scenario"}, {"value": "0.02570207357735", "module": "A5", "scenario": "Standard scenario"}, {"value": "0.01003459350362", "module": "C1", "scenario": "Standard scenario"}, {"value": "0.0571206860608", "module": "C2", "scenario": "Standard scenario"}, {"value": "6.14090146625", "module": "C3", "scenario": "Standard scenario"}, {"value": "0.011363403", "module": "C4", "scenario": "Standard scenario"}, {"value": "-34.1877086332943", "module": "D", "scenario": "Standard scenario"}, {"name": "referenceToUnitGroupDataSet", "value": {"shortDescription": [{"value": "MJ", "lang": "en"}], "type": "unit group data set", "refObjectId": "93a60a57-a3c8-11da-a746-0800200c9a66", "version": "03.00.000", "uri": "../unitgroups/93a60a57-a3c8-11da-a746-0800200c9a66.xml"}}]}, "flowProperties": [], "typeOfFlow": "Other flow", "classification": {"classHierarchy": "Quantities", "name": "GaBiCategories"}}, {"dataSetInternalID": 15, "referenceToFlowDataSet": {"shortDescription": [{"value": "Use of renewable primary energy resources used as raw materials (PERM)", "lang": "en"}, {"value": "Erneuerbare Primärenergie zur stofflichen Nutzung (PERM)", "lang": "de"}, {"value": "Uso de energía primaria renovable utilizada como materia prima (PERM)", "lang": "es"}], "type": "flow data set", "refObjectId": "fb3ec0de-548d-4508-aea5-00b73bf6f702", "version": "38.00.000", "uri": "../flows/fb3ec0de-548d-4508-aea5-00b73bf6f702.xml"}, "exchange direction": "INPUT", "meanAmount": 0.0, "other": {"anies": [{"value": "0.0", "module": "A1", "scenario": "Standard scenario"}, {"value": "0.0", "module": "A2", "scenario": "Standard scenario"}, {"value": "38.4725", "module": "A3", "scenario": "Standard scenario"}, {"value": "38.4725", "module": "A1-A3", "scenario": "Standard scenario"}, {"value": "0.0", "module": "A5", "scenario": "Standard scenario"}, {"value": "0.0", "module": "C1", "scenario": "Standard scenario"}, {"value": "0.0", "module": "C2", "scenario": "Standard scenario"}, {"value": "0.0", "module": "C3", "scenario": "Standard scenario"}, {"value": "0.0", "module": "C4", "scenario": "Standard scenario"}, {"value": "0.0", "module": "D", "scenario": "Standard scenario"}, {"name": "referenceToUnitGroupDataSet", "value": {"shortDescription": [{"value": "MJ", "lang": "en"}], "type": "unit group data set", "refObjectId": "93a60a57-a3c8-11da-a746-0800200c9a66", "version": "03.00.000", "uri": "../unitgroups/93a60a57-a3c8-11da-a746-0800200c9a66.xml"}}]}, "flowProperties": [], "typeOfFlow": "Other flow", "classification": {"classHierarchy": "Quantities", "name": "GaBiCategories"}}, {"dataSetInternalID": 16, "referenceToFlowDataSet": {"shortDescription": [{"value": "Total use of renewable primary energy resources (PERT)", "lang": "en"}, {"value": "Total erneuerbare Primärenergie (PERT)", "lang": "de"}, {"value": "Uso total de la energía primaria renovable (energía primaria y recursos de energía primaria renovable utilizada como materia prima) (PERT)", "lang": "es"}], "type": "flow data set", "refObjectId": "53f97275-fa8a-4cdd-9024-65936002acd0", "version": "30.00.000", "uri": "../flows/53f97275-fa8a-4cdd-9024-65936002acd0.xml"}, "exchange direction": "INPUT", "meanAmount": 0.0, "other": {"anies": [{"value": "40.3988699534339", "module": "A1", "scenario": "Standard scenario"}, {"value": "0.12441228200141", "module": "A2", "scenario": "Standard scenario"}, {"value": "81.7038738226156", "module": "A3", "scenario": "Standard scenario"}, {"value": "122.22715605805092", "module": "A1-A3", "scenario": "Standard scenario"}, {"value": "0.02570207357735", "module": "A5", "scenario": "Standard scenario"}, {"value": "0.01003459350362", "module": "C1", "scenario": "Standard scenario"}, {"value": "0.0571206860608", "module": "C2", "scenario": "Standard scenario"}, {"value": "6.14090146625", "module": "C3", "scenario": "Standard scenario"}, {"value": "0.011363403", "module": "C4", "scenario": "Standard scenario"}, {"value": "-34.1877086332943", "module": "D", "scenario": "Standard scenario"}, {"name": "referenceToUnitGroupDataSet", "value": {"shortDescription": [{"value": "MJ", "lang": "en"}], "type": "unit group data set", "refObjectId": "93a60a57-a3c8-11da-a746-0800200c9a66", "version": "03.00.000", "uri": "../unitgroups/93a60a57-a3c8-11da-a746-0800200c9a66.xml"}}]}, "flowProperties": [], "typeOfFlow": "Other flow", "classification": {"classHierarchy": "Größen / Umweltliche Größen / EPD EN 15804 / LCI Indikatoren", "name": "GaBiCategories"}}, {"dataSetInternalID": 17, "referenceToFlowDataSet": {"shortDescription": [{"value": "Use of renewable secondary fuels (RSF)", "lang": "en"}, {"value": "Erneuerbare Sekundärbrennstoffe (RSF)", "lang": "de"}, {"value": "Uso de combustibles secundarios renovables (RSF)", "lang": "es"}], "type": "flow data set", "refObjectId": "64333088-a55f-4aa2-9a31-c10b07816787", "version": "30.00.000", "uri": "../flows/64333088-a55f-4aa2-9a31-c10b07816787.xml"}, "exchange direction": "INPUT", "meanAmount": 0.0, "other": {"anies": [{"value": "0.0", "module": "A1", "scenario": "Standard scenario"}, {"value": "0.0", "module": "A2", "scenario": "Standard scenario"}, {"value": "0.0", "module": "A3", "scenario": "Standard scenario"}, {"value": "0.0", "module": "A1-A3", "scenario": "Standard scenario"}, {"value": "0.0", "module": "A5", "scenario": "Standard scenario"}, {"value": "0.0", "module": "C1", "scenario": "Standard scenario"}, {"value": "0.0", "module": "C2", "scenario": "Standard scenario"}, {"value": "0.0", "module": "C3", "scenario": "Standard scenario"}, {"value": "0.0", "module": "C4", "scenario": "Standard scenario"}, {"value": "0.0", "module": "D", "scenario": "Standard scenario"}, {"name": "referenceToUnitGroupDataSet", "value": {"shortDescription": [{"value": "MJ", "lang": "en"}], "type": "unit group data set", "refObjectId": "93a60a57-a3c8-11da-a746-0800200c9a66", "version": "03.00.000", "uri": "../unitgroups/93a60a57-a3c8-11da-a746-0800200c9a66.xml"}}]}, "flowProperties": [], "typeOfFlow": "Other flow", "classification": {"classHierarchy": "Größen / Umweltliche Größen / EPD EN 15804 / LCI Indikatoren", "name": "GaBiCategories"}}, {"dataSetInternalID": 18, "referenceToFlowDataSet": {"shortDescription": [{"value": "Radioactive waste disposed (RWD)", "lang": "en"}, {"value": "Entsorgter radioaktiver Abfall (RWD)", "lang": "de"}, {"value": "Residuos radiactivos eliminados (RWD)", "lang": "es"}], "type": "flow data set", "refObjectId": "3449546e-52ad-4b39-b809-9fb77cea8ff6", "version": "30.00.000", "uri": "../flows/3449546e-52ad-4b39-b809-9fb77cea8ff6.xml"}, "exchange direction": "OUTPUT", "meanAmount": 0.0, "other": {"anies": [{"value": "0.00171950565622", "module": "A1", "scenario": "Standard scenario"}, {"value": "6.525649685E-5", "module": "A2", "scenario": "Standard scenario"}, {"value": "9.154347421E-5", "module": "A3", "scenario": "Standard scenario"}, {"value": "0.00187630562728", "module": "A1-A3", "scenario": "Standard scenario"}, {"value": "6.44901395E-6", "module": "A5", "scenario": "Standard scenario"}, {"value": "1.288166043E-5", "module": "C1", "scenario": "Standard scenario"}, {"value": "2.996083514E-5", "module": "C2", "scenario": "Standard scenario"}, {"value": "3.670161375E-4", "module": "C3", "scenario": "Standard scenario"}, {"value": "3.9881564E-6", "module": "C4", "scenario": "Standard scenario"}, {"value": "5.247330361E-5", "module": "D", "scenario": "Standard scenario"}, {"name": "referenceToUnitGroupDataSet", "value": {"shortDescription": [{"value": "kg", "lang": "en"}], "type": "unit group data set", "refObjectId": "ad38d542-3fe9-439d-9b95-2f5f7752acaf", "version": "30.00.000", "uri": "../unitgroups/ad38d542-3fe9-439d-9b95-2f5f7752acaf.xml"}}]}, "flowProperties": [], "typeOfFlow": "Other flow", "classification": {"classHierarchy": "Größen / Umweltliche Größen / EPD EN 15804 / LCI Indikatoren", "name": "GaBiCategories"}}, {"dataSetInternalID": 19, "referenceToFlowDataSet": {"shortDescription": [{"value": "Use of secondary material (SM)", "lang": "en"}, {"value": "Einsatz von Sekundärstoffen (SM)", "lang": "de"}, {"value": "Uso de materiales secundarios (SM)", "lang": "es"}], "type": "flow data set", "refObjectId": "c6a1f35f-2d09-4f54-8dfb-97e502e1ce92", "version": "30.00.000", "uri": "../flows/c6a1f35f-2d09-4f54-8dfb-97e502e1ce92.xml"}, "exchange direction": "INPUT", "meanAmount": 0.0, "other": {"anies": [{"value": "28.0513524936601", "module": "A1", "scenario": "Standard scenario"}, {"value": "0.0", "module": "A2", "scenario": "Standard scenario"}, {"value": "0.02076794167371", "module": "A3", "scenario": "Standard scenario"}, {"value": "28.07212043533381", "module": "A1-A3", "scenario": "Standard scenario"}, {"value": "0.0", "module": "A5", "scenario": "Standard scenario"}, {"value": "0.0", "module": "C1", "scenario": "Standard scenario"}, {"value": "0.0", "module": "C2", "scenario": "Standard scenario"}, {"value": "0.0", "module": "C3", "scenario": "Standard scenario"}, {"value": "0.0", "module": "C4", "scenario": "Standard scenario"}, {"value": "0.0", "module": "D", "scenario": "Standard scenario"}, {"name": "referenceToUnitGroupDataSet", "value": {"shortDescription": [{"value": "kg", "lang": "en"}], "type": "unit group data set", "refObjectId": "ad38d542-3fe9-439d-9b95-2f5f7752acaf", "version": "30.00.000", "uri": "../unitgroups/ad38d542-3fe9-439d-9b95-2f5f7752acaf.xml"}}]}, "flowProperties": [], "typeOfFlow": "Other flow", "classification": {"classHierarchy": "Größen / Umweltliche Größen / EPD EN 15804 / LCI Indikatoren", "name": "GaBiCategories"}}]}, "LCIAResults": {"LCIAResult": [{"referenceToLCIAMethodDataSet": {"shortDescription": [{"value": "Abiotic depletion potential - non-fossil resources (ADPE)", "lang": "en"}, {"value": "Potenzial für die Verknappung abiotischer Ressourcen – nicht fossile Ressourcen (ADPE)", "lang": "de"}], "type": "LCIA method data set", "refObjectId": "b2ad6494-c78d-11e6-9d9d-cec0c932ce01", "version": "01.00.011", "uri": "../lciamethods/b2ad6494-c78d-11e6-9d9d-cec0c932ce01.xml"}, "meanAmount": 0.0, "other": {"anies": [{"value": "6.5780459903E-4", "module": "A1", "scenario": "Standard scenario"}, {"value": "1.66947305E-5", "module": "A2", "scenario": "Standard scenario"}, {"value": "2.512434866E-5", "module": "A3", "scenario": "Standard scenario"}, {"value": "6.996236781900001E-4", "module": "A1-A3", "scenario": "Standard scenario"}, {"value": "1.46626064E-6", "module": "A5", "scenario": "Standard scenario"}, {"value": "2.0672155E-7", "module": "C1", "scenario": "Standard scenario"}, {"value": "7.66495433E-6", "module": "C2", "scenario": "Standard scenario"}, {"value": "1.32463975E-4", "module": "C3", "scenario": "Standard scenario"}, {"value": "2.9958694E-7", "module": "C4", "scenario": "Standard scenario"}, {"value": "-1.093307311E-5", "module": "D", "scenario": "Standard scenario"}, {"name": "referenceToUnitGroupDataSet", "value": {"shortDescription": [{"value": "kg Sb-eq.", "lang": "en"}], "type": "unit group data set", "refObjectId": "54ccd2d9-a32a-4fc2-923d-f2c8c93e89d4", "version": "30.00.000", "uri": "../unitgroups/54ccd2d9-a32a-4fc2-923d-f2c8c93e89d4.xml"}}]}}, {"referenceToLCIAMethodDataSet": {"shortDescription": [{"value": "Abiotic depletion potential - fossil resources (ADPF)", "lang": "en"}, {"value": "Potenzial für die Verknappung abiotischer Ressourcen – fossile Brennstoffe (ADPF)", "lang": "de"}], "type": "LCIA method data set", "refObjectId": "b2ad6110-c78d-11e6-9d9d-cec0c932ce01", "version": "01.00.011", "uri": "../lciamethods/b2ad6110-c78d-11e6-9d9d-cec0c932ce01.xml"}, "meanAmount": 0.0, "other": {"anies": [{"value": "475.236230696635", "module": "A1", "scenario": "Standard scenario"}, {"value": "9.93764775305906", "module": "A2", "scenario": "Standard scenario"}, {"value": "29.1147672579468", "module": "A3", "scenario": "Standard scenario"}, {"value": "514.2886457076409", "module": "A1-A3", "scenario": "Standard scenario"}, {"value": "1.10110717371675", "module": "A5", "scenario": "Standard scenario"}, {"value": "1.8551732058859", "module": "C1", "scenario": "Standard scenario"}, {"value": "4.56261430426042", "module": "C2", "scenario": "Standard scenario"}, {"value": "97.09077757", "module": "C3", "scenario": "Standard scenario"}, {"value": "0.6672889489", "module": "C4", "scenario": "Standard scenario"}, {"value": "-98.8105540041154", "module": "D", "scenario": "Standard scenario"}, {"name": "referenceToUnitGroupDataSet", "value": {"shortDescription": [{"value": "MJ", "lang": "en"}], "type": "unit group data set", "refObjectId": "93a60a57-a3c8-11da-a746-0800200c9a66", "version": "03.00.000", "uri": "../unitgroups/93a60a57-a3c8-11da-a746-0800200c9a66.xml"}}]}}, {"referenceToLCIAMethodDataSet": {"shortDescription": [{"value": "Acidification potential, Accumulated Exceedance (AP)", "lang": "en"}, {"value": "Versauerungspotenzial, kumulierte Überschreitung (AP)", "lang": "de"}], "type": "LCIA method data set", "refObjectId": "b5c611c6-def3-11e6-bf01-fe55135034f3", "version": "01.03.010", "uri": "../lciamethods/b5c611c6-def3-11e6-bf01-fe55135034f3.xml"}, "meanAmount": 0.0, "other": {"anies": [{"value": "0.17375936397329", "module": "A1", "scenario": "Standard scenario"}, {"value": "0.00382149420403", "module": "A2", "scenario": "Standard scenario"}, {"value": "0.00858150297459", "module": "A3", "scenario": "Standard scenario"}, {"value": "0.18616236115191", "module": "A1-A3", "scenario": "Standard scenario"}, {"value": "0.00106715650726", "module": "A5", "scenario": "Standard scenario"}, {"value": "0.00140982831094", "module": "C1", "scenario": "Standard scenario"}, {"value": "0.00175454036531", "module": "C2", "scenario": "Standard scenario"}, {"value": "0.03254362125", "module": "C3", "scenario": "Standard scenario"}, {"value": "2.4774125E-4", "module": "C4", "scenario": "Standard scenario"}, {"value": "-0.05722388843116", "module": "D", "scenario": "Standard scenario"}, {"name": "referenceToUnitGroupDataSet", "value": {"shortDescription": [{"value": "mol H+-eq.", "lang": "en"}], "type": "unit group data set", "refObjectId": "42e089ac-92bf-4bf2-8ca1-5fc40d18f2ed", "version": "00.01.000", "uri": "../unitgroups/42e089ac-92bf-4bf2-8ca1-5fc40d18f2ed.xml"}}]}}, {"referenceToLCIAMethodDataSet": {"shortDescription": [{"value": "Eutrophication potential - freshwater (EP-freshwater)", "lang": "en"}, {"value": "Eutrophierungspotenzial - Süßwasser (EP-freshwater)", "lang": "de"}], "type": "LCIA method data set", "refObjectId": "b53ec18f-7377-4ad3-86eb-cc3f4f276b2b", "version": "01.00.011", "uri": "../lciamethods/b53ec18f-7377-4ad3-86eb-cc3f4f276b2b.xml"}, "meanAmount": 0.0, "other": {"anies": [{"value": "0.00211219975303", "module": "A1", "scenario": "Standard scenario"}, {"value": "6.64682625E-6", "module": "A2", "scenario": "Standard scenario"}, {"value": "8.360766453E-5", "module": "A3", "scenario": "Standard scenario"}, {"value": "0.00220245424381", "module": "A1-A3", "scenario": "Standard scenario"}, {"value": "1.15799427E-6", "module": "A5", "scenario": "Standard scenario"}, {"value": "4.9071032E-7", "module": "C1", "scenario": "Standard scenario"}, {"value": "3.0517186E-6", "module": "C2", "scenario": "Standard scenario"}, {"value": "2.182582875E-4", "module": "C3", "scenario": "Standard scenario"}, {"value": "4.908128E-7", "module": "C4", "scenario": "Standard scenario"}, {"value": "-4.9926267178E-4", "module": "D", "scenario": "Standard scenario"}, {"name": "referenceToUnitGroupDataSet", "value": {"shortDescription": [{"value": "kg P-eq.", "lang": "en"}], "type": "unit group data set", "refObjectId": "0429039d-a61d-4590-ba67-aa4a20a810a1", "version": "30.00.000", "uri": "../unitgroups/0429039d-a61d-4590-ba67-aa4a20a810a1.xml"}}]}}, {"referenceToLCIAMethodDataSet": {"shortDescription": [{"value": "Eutrophication potential - marine (EP-marine)", "lang": "en"}, {"value": "Eutrophierungspotenzial - Salzwasser (EP-marine)", "lang": "de"}], "type": "LCIA method data set", "refObjectId": "b5c619fa-def3-11e6-bf01-fe55135034f3", "version": "02.00.011", "uri": "../lciamethods/b5c619fa-def3-11e6-bf01-fe55135034f3.xml"}, "meanAmount": 0.0, "other": {"anies": [{"value": "0.03473566273834", "module": "A1", "scenario": "Standard scenario"}, {"value": "0.00134660291451", "module": "A2", "scenario": "Standard scenario"}, {"value": "0.00212422969577", "module": "A3", "scenario": "Standard scenario"}, {"value": "0.03820649534862", "module": "A1-A3", "scenario": "Standard scenario"}, {"value": "4.6360370219E-4", "module": "A5", "scenario": "Standard scenario"}, {"value": "6.2237763992E-4", "module": "C1", "scenario": "Standard scenario"}, {"value": "6.1825794922E-4", "module": "C2", "scenario": "Standard scenario"}, {"value": "0.0082307525", "module": "C3", "scenario": "Standard scenario"}, {"value": "1.3548424E-4", "module": "C4", "scenario": "Standard scenario"}, {"value": "-0.01105447383328", "module": "D", "scenario": "Standard scenario"}, {"name": "referenceToUnitGroupDataSet", "value": {"shortDescription": [{"value": "kg N-eq.", "lang": "en"}], "type": "unit group data set", "refObjectId": "d05bb823-ecdf-4686-8c40-bf1d9257859f", "version": "00.00.003", "uri": "../unitgroups/d05bb823-ecdf-4686-8c40-bf1d9257859f.xml"}}]}}, {"referenceToLCIAMethodDataSet": {"shortDescription": [{"value": "Eutrophication potential - terrestrial (EP-terrestrial)", "lang": "en"}, {"value": "Eutrophierungspotenzial - Land (EP-terrestrial)", "lang": "de"}], "type": "LCIA method data set", "refObjectId": "b5c614d2-def3-11e6-bf01-fe55135034f3", "version": "01.02.010", "uri": "../lciamethods/b5c614d2-def3-11e6-bf01-fe55135034f3.xml"}, "meanAmount": 0.0, "other": {"anies": [{"value": "0.36049378478719", "module": "A1", "scenario": "Standard scenario"}, {"value": "0.0148464544008", "module": "A2", "scenario": "Standard scenario"}, {"value": "0.0238006714803", "module": "A3", "scenario": "Standard scenario"}, {"value": "0.39914091066829005", "module": "A1-A3", "scenario": "Standard scenario"}, {"value": "0.00518304603618", "module": "A5", "scenario": "Standard scenario"}, {"value": "0.00682892129244", "module": "C1", "scenario": "Standard scenario"}, {"value": "0.00681636609587", "module": "C2", "scenario": "Standard scenario"}, {"value": "0.0905911775", "module": "C3", "scenario": "Standard scenario"}, {"value": "9.03948E-4", "module": "C4", "scenario": "Standard scenario"}, {"value": "-0.13532685051908", "module": "D", "scenario": "Standard scenario"}, {"name": "referenceToUnitGroupDataSet", "value": {"shortDescription": [{"value": "mol N-eq.", "lang": "en"}], "type": "unit group data set", "refObjectId": "71b4d617-0ec9-4d3f-b65e-e438940c2401", "version": "00.00.003", "uri": "../unitgroups/71b4d617-0ec9-4d3f-b65e-e438940c2401.xml"}}]}}, {"referenceToLCIAMethodDataSet": {"shortDescription": [{"value": "Potential Comparative Toxic Unit for ecosystems (ETP-fw)", "lang": "en"}, {"value": "Potenzielle Toxizitätsvergleichseinheit für Ökosysteme (ETP-fw)", "lang": "de"}], "type": "LCIA method data set", "refObjectId": "05316e7a-b254-4bea-9cf0-6bf33eb5c630", "version": "01.00.003", "uri": "../lciamethods/05316e7a-b254-4bea-9cf0-6bf33eb5c630.xml"}, "meanAmount": 0.0, "other": {"anies": [{"value": "1155.34245051721", "module": "A1", "scenario": "Standard scenario"}, {"value": "8.86161044183438", "module": "A2", "scenario": "Standard scenario"}, {"value": "36.022618548672", "module": "A3", "scenario": "Standard scenario"}, {"value": "1200.2266795077162", "module": "A1-A3", "scenario": "Standard scenario"}, {"value": "1.30341397720806", "module": "A5", "scenario": "Standard scenario"}, {"value": "1.1183379971464", "module": "C1", "scenario": "Standard scenario"}, {"value": "4.06857956383601", "module": "C2", "scenario": "Standard scenario"}, {"value": "490.99898112", "module": "C3", "scenario": "Standard scenario"}, {"value": "10.0588262433", "module": "C4", "scenario": "Standard scenario"}, {"value": "-492.951505738271", "module": "D", "scenario": "Standard scenario"}, {"name": "referenceToUnitGroupDataSet", "value": {"shortDescription": [{"value": "CTUe", "lang": "en"}], "type": "unit group data set", "refObjectId": "aa959ded-f1eb-4efb-9c5c-2d60be36b3e6", "version": "00.00.003", "uri": "../unitgroups/aa959ded-f1eb-4efb-9c5c-2d60be36b3e6.xml"}}]}}, {"referenceToLCIAMethodDataSet": {"shortDescription": [{"value": "Global Warming Potential - biogenic (GWP-biogenic)", "lang": "en"}, {"value": "Globales Erwärmungspotenzial - biogen (GWP-biogenic)", "lang": "de"}], "type": "LCIA method data set", "refObjectId": "a7ea186c-9749-11ed-a8fc-0242ac120002", "version": "01.00.006", "uri": "../lciamethods/a7ea186c-9749-11ed-a8fc-0242ac120002.xml"}, "meanAmount": 0.0, "other": {"anies": [{"value": "1.56927352185079", "module": "A1", "scenario": "Standard scenario"}, {"value": "3.0418418487E-4", "module": "A2", "scenario": "Standard scenario"}, {"value": "-4.57042851289527", "module": "A3", "scenario": "Standard scenario"}, {"value": "-3.00085080685961", "module": "A1-A3", "scenario": "Standard scenario"}, {"value": "4.6065304579433", "module": "A5", "scenario": "Standard scenario"}, {"value": "3.748936726E-5", "module": "C1", "scenario": "Standard scenario"}, {"value": "1.3965831226E-4", "module": "C2", "scenario": "Standard scenario"}, {"value": "-1.57", "module": "C3", "scenario": "Standard scenario"}, {"value": "2.9787268E-4", "module": "C4", "scenario": "Standard scenario"}, {"value": "0.13656037009076", "module": "D", "scenario": "Standard scenario"}, {"name": "referenceToUnitGroupDataSet", "value": {"shortDescription": [{"value": "kg CO2-eq.", "lang": "en"}], "type": "unit group data set", "refObjectId": "1ebf3012-d0db-4de2-aefd-ef30cedb0be1", "version": "30.00.000", "uri": "../unitgroups/1ebf3012-d0db-4de2-aefd-ef30cedb0be1.xml"}}]}}, {"referenceToLCIAMethodDataSet": {"shortDescription": [{"value": "Global Warming Potential - fossil fuels (GWP-fossil)", "lang": "en"}, {"value": "Globales Erwärmungspotenzial - fossil (GWP-fossil)", "lang": "de"}], "type": "LCIA method data set", "refObjectId": "a7ea19c0-9749-11ed-a8fc-0242ac120002", "version": "01.00.009", "uri": "../lciamethods/a7ea19c0-9749-11ed-a8fc-0242ac120002.xml"}, "meanAmount": 0.0, "other": {"anies": [{"value": "39.1550770358816", "module": "A1", "scenario": "Standard scenario"}, {"value": "0.65890823874764", "module": "A2", "scenario": "Standard scenario"}, {"value": "1.81685980103858", "module": "A3", "scenario": "Standard scenario"}, {"value": "41.63084507566782", "module": "A1-A3", "scenario": "Standard scenario"}, {"value": "0.07739479839031", "module": "A5", "scenario": "Standard scenario"}, {"value": "0.13479152260771", "module": "C1", "scenario": "Standard scenario"}, {"value": "0.30252070007005", "module": "C2", "scenario": "Standard scenario"}, {"value": "13.781385685", "module": "C3", "scenario": "Standard scenario"}, {"value": "0.2199779022", "module": "C4", "scenario": "Standard scenario"}, {"value": "-13.6333281654973", "module": "D", "scenario": "Standard scenario"}, {"name": "referenceToUnitGroupDataSet", "value": {"shortDescription": [{"value": "kg CO2-eq.", "lang": "en"}], "type": "unit group data set", "refObjectId": "1ebf3012-d0db-4de2-aefd-ef30cedb0be1", "version": "30.00.000", "uri": "../unitgroups/1ebf3012-d0db-4de2-aefd-ef30cedb0be1.xml"}}]}}, {"referenceToLCIAMethodDataSet": {"shortDescription": [{"value": "Global Warming Potential - land use and land use change (GWP-luluc)", "lang": "en"}, {"value": "Globales Erwärmungspotenzial - luluc (GWP-luluc)", "lang": "de"}], "type": "LCIA method data set", "refObjectId": "a7ea1ae2-9749-11ed-a8fc-0242ac120002", "version": "01.00.006", "uri": "../lciamethods/a7ea1ae2-9749-11ed-a8fc-0242ac120002.xml"}, "meanAmount": 0.0, "other": {"anies": [{"value": "0.02454208992707", "module": "A1", "scenario": "Standard scenario"}, {"value": "2.4144619318E-4", "module": "A2", "scenario": "Standard scenario"}, {"value": "0.00381442417131", "module": "A3", "scenario": "Standard scenario"}, {"value": "0.02859796029156", "module": "A1-A3", "scenario": "Standard scenario"}, {"value": "2.911859782E-5", "module": "A5", "scenario": "Standard scenario"}, {"value": "1.062339241E-5", "module": "C1", "scenario": "Standard scenario"}, {"value": "1.1085378372E-4", "module": "C2", "scenario": "Standard scenario"}, {"value": "0.00686597625", "module": "C3", "scenario": "Standard scenario"}, {"value": "1.3388974E-5", "module": "C4", "scenario": "Standard scenario"}, {"value": "0.00754875118295", "module": "D", "scenario": "Standard scenario"}, {"name": "referenceToUnitGroupDataSet", "value": {"shortDescription": [{"value": "kg CO2-eq.", "lang": "en"}], "type": "unit group data set", "refObjectId": "1ebf3012-d0db-4de2-aefd-ef30cedb0be1", "version": "30.00.000", "uri": "../unitgroups/1ebf3012-d0db-4de2-aefd-ef30cedb0be1.xml"}}]}}, {"referenceToLCIAMethodDataSet": {"shortDescription": [{"value": "Global Warming Potential - total (GWP-total)", "lang": "en"}, {"value": "Globales Erwärmungspotenzial - total (GWP-total)", "lang": "de"}], "type": "LCIA method data set", "refObjectId": "a7ea142a-9749-11ed-a8fc-0242ac120002", "version": "04.00.017", "uri": "../lciamethods/a7ea142a-9749-11ed-a8fc-0242ac120002.xml"}, "meanAmount": 0.0, "other": {"anies": [{"value": "40.7488926476599", "module": "A1", "scenario": "Standard scenario"}, {"value": "0.65945386912567", "module": "A2", "scenario": "Standard scenario"}, {"value": "-2.74974878957715", "module": "A3", "scenario": "Standard scenario"}, {"value": "38.658597727208424", "module": "A1-A3", "scenario": "Standard scenario"}, {"value": "4.68395360818641", "module": "A5", "scenario": "Standard scenario"}, {"value": "0.13483963536738", "module": "C1", "scenario": "Standard scenario"}, {"value": "0.30277121216603", "module": "C2", "scenario": "Standard scenario"}, {"value": "12.2", "module": "C3", "scenario": "Standard scenario"}, {"value": "0.2202888584", "module": "C4", "scenario": "Standard scenario"}, {"value": "-13.4891748669683", "module": "D", "scenario": "Standard scenario"}, {"name": "referenceToUnitGroupDataSet", "value": {"shortDescription": [{"value": "kg CO2-eq.", "lang": "en"}], "type": "unit group data set", "refObjectId": "1ebf3012-d0db-4de2-aefd-ef30cedb0be1", "version": "30.00.000", "uri": "../unitgroups/1ebf3012-d0db-4de2-aefd-ef30cedb0be1.xml"}}]}}, {"referenceToLCIAMethodDataSet": {"shortDescription": [{"value": "Potential Comparative Toxic Unit for humans - cancer effects (HTP-c)", "lang": "en"}, {"value": "Potenzielle Toxizitätsvergleichseinheit für den Menschen - kanzerogene Wirkung (HTP-c)", "lang": "de"}], "type": "LCIA method data set", "refObjectId": "2299222a-bbd8-474f-9d4f-4dd1f18aea7c", "version": "01.00.004", "uri": "../lciamethods/2299222a-bbd8-474f-9d4f-4dd1f18aea7c.xml"}, "meanAmount": 0.0, "other": {"anies": [{"value": "1.5565223E-7", "module": "A1", "scenario": "Standard scenario"}, {"value": "2.8742E-10", "module": "A2", "scenario": "Standard scenario"}, {"value": "4.36117E-9", "module": "A3", "scenario": "Standard scenario"}, {"value": "1.6030082E-7", "module": "A1-A3", "scenario": "Standard scenario"}, {"value": "7.1481E-10", "module": "A5", "scenario": "Standard scenario"}, {"value": "3.908E-11", "module": "C1", "scenario": "Standard scenario"}, {"value": "1.3196E-10", "module": "C2", "scenario": "Standard scenario"}, {"value": "1.021842E-8", "module": "C3", "scenario": "Standard scenario"}, {"value": "1.961E-11", "module": "C4", "scenario": "Standard scenario"}, {"value": "-6.5887E-9", "module": "D", "scenario": "Standard scenario"}, {"name": "referenceToUnitGroupDataSet", "value": {"shortDescription": [{"value": "CTUh", "lang": "en"}], "type": "unit group data set", "refObjectId": "d4c9523e-2d7e-49fd-8469-998f547d3a70", "version": "00.00.003", "uri": "../unitgroups/d4c9523e-2d7e-49fd-8469-998f547d3a70.xml"}}]}}, {"referenceToLCIAMethodDataSet": {"shortDescription": [{"value": "Potential Comparative Toxic Unit for humans - non-cancer effects (HTP-nc)", "lang": "en"}, {"value": "Potenzielle Toxizitätsvergleichseinheit für den Menschen - nicht kanzerogene Wirkung (HTP-nc)", "lang": "de"}], "type": "LCIA method data set", "refObjectId": "7cfdcfcf-b222-4b26-888a-a55f9fbf7ac8", "version": "01.00.003", "uri": "../lciamethods/7cfdcfcf-b222-4b26-888a-a55f9fbf7ac8.xml"}, "meanAmount": 0.0, "other": {"anies": [{"value": "1.36997296E-6", "module": "A1", "scenario": "Standard scenario"}, {"value": "9.69327E-9", "module": "A2", "scenario": "Standard scenario"}, {"value": "3.83726E-8", "module": "A3", "scenario": "Standard scenario"}, {"value": "1.41803883E-6", "module": "A1-A3", "scenario": "Standard scenario"}, {"value": "3.03871E-9", "module": "A5", "scenario": "Standard scenario"}, {"value": "9.6037E-10", "module": "C1", "scenario": "Standard scenario"}, {"value": "4.45041E-9", "module": "C2", "scenario": "Standard scenario"}, {"value": "2.1300966E-7", "module": "C3", "scenario": "Standard scenario"}, {"value": "2.00239E-9", "module": "C4", "scenario": "Standard scenario"}, {"value": "2.43585581E-6", "module": "D", "scenario": "Standard scenario"}, {"name": "referenceToUnitGroupDataSet", "value": {"shortDescription": [{"value": "CTUh", "lang": "en"}], "type": "unit group data set", "refObjectId": "d4c9523e-2d7e-49fd-8469-998f547d3a70", "version": "00.00.003", "uri": "../unitgroups/d4c9523e-2d7e-49fd-8469-998f547d3a70.xml"}}]}}, {"referenceToLCIAMethodDataSet": {"shortDescription": [{"value": "Potential Human exposure efficiency relative to U235 (IRP)", "lang": "en"}, {"value": "Potenzielle Wirkung durch Exposition des Menschen mit U235 (IRP)", "lang": "de"}], "type": "LCIA method data set", "refObjectId": "b5c632be-def3-11e6-bf01-fe55135034f3", "version": "01.00.012", "uri": "../lciamethods/b5c632be-def3-11e6-bf01-fe55135034f3.xml"}, "meanAmount": 0.0, "other": {"anies": [{"value": "1.77404010601369", "module": "A1", "scenario": "Standard scenario"}, {"value": "0.04163729155808", "module": "A2", "scenario": "Standard scenario"}, {"value": "0.07895347178947", "module": "A3", "scenario": "Standard scenario"}, {"value": "1.8946308693612401", "module": "A1-A3", "scenario": "Standard scenario"}, {"value": "0.00435012295925", "module": "A5", "scenario": "Standard scenario"}, {"value": "0.00794982753806", "module": "C1", "scenario": "Standard scenario"}, {"value": "0.01911668704449", "module": "C2", "scenario": "Standard scenario"}, {"value": "0.32131279", "module": "C3", "scenario": "Standard scenario"}, {"value": "0.0026142318", "module": "C4", "scenario": "Standard scenario"}, {"value": "0.19989276790193", "module": "D", "scenario": "Standard scenario"}, {"name": "referenceToUnitGroupDataSet", "value": {"shortDescription": [{"value": "kgBq U235-eq.", "lang": "en"}], "type": "unit group data set", "refObjectId": "456b05bf-1415-44a9-9993-02452f554c09", "version": "00.00.003", "uri": "../unitgroups/456b05bf-1415-44a9-9993-02452f554c09.xml"}}]}}, {"referenceToLCIAMethodDataSet": {"shortDescription": [{"value": "Depletion potential of the stratospheric ozone layer (ODP)", "lang": "en"}, {"value": "Abbaupotenzial der stratosphärischen Ozonschicht (ODP)", "lang": "de"}], "type": "LCIA method data set", "refObjectId": "b5c629d6-def3-11e6-bf01-fe55135034f3", "version": "02.00.013", "uri": "../lciamethods/b5c629d6-def3-11e6-bf01-fe55135034f3.xml"}, "meanAmount": 0.0, "other": {"anies": [{"value": "2.85760667E-6", "module": "A1", "scenario": "Standard scenario"}, {"value": "1.4543687E-7", "module": "A2", "scenario": "Standard scenario"}, {"value": "1.6195644E-7", "module": "A3", "scenario": "Standard scenario"}, {"value": "3.1649999799999997E-6", "module": "A1-A3", "scenario": "Standard scenario"}, {"value": "1.525601E-8", "module": "A5", "scenario": "Standard scenario"}, {"value": "2.910953E-8", "module": "C1", "scenario": "Standard scenario"}, {"value": "6.677358E-8", "module": "C2", "scenario": "Standard scenario"}, {"value": "1.53937563E-6", "module": "C3", "scenario": "Standard scenario"}, {"value": "8.78401E-9", "module": "C4", "scenario": "Standard scenario"}, {"value": "-3.9144389E-7", "module": "D", "scenario": "Standard scenario"}, {"name": "referenceToUnitGroupDataSet", "value": {"shortDescription": [{"value": "kg CFC-11-eq.", "lang": "en"}], "type": "unit group data set", "refObjectId": "d9e957c9-7309-4474-bf3a-7777df6c4e5b", "version": "25.00.000", "uri": "../unitgroups/d9e957c9-7309-4474-bf3a-7777df6c4e5b.xml"}}]}}, {"referenceToLCIAMethodDataSet": {"shortDescription": [{"value": "Potential incidence of disease due to PM emissions (PM)", "lang": "en"}, {"value": "Potenzielles Auftreten von Krankheiten aufgrund von Feinstaubemissionen (PM)", "lang": "de"}], "type": "LCIA method data set", "refObjectId": "b5c602c6-def3-11e6-bf01-fe55135034f3", "version": "02.00.012", "uri": "../lciamethods/b5c602c6-def3-11e6-bf01-fe55135034f3.xml"}, "meanAmount": 0.0, "other": {"anies": [{"value": "2.54794649E-6", "module": "A1", "scenario": "Standard scenario"}, {"value": "5.927775E-8", "module": "A2", "scenario": "Standard scenario"}, {"value": "1.6171717E-7", "module": "A3", "scenario": "Standard scenario"}, {"value": "2.76894141E-6", "module": "A1-A3", "scenario": "Standard scenario"}, {"value": "1.112272E-8", "module": "A5", "scenario": "Standard scenario"}, {"value": "3.737151E-8", "module": "C1", "scenario": "Standard scenario"}, {"value": "2.721585E-8", "module": "C2", "scenario": "Standard scenario"}, {"value": "4.5962329E-7", "module": "C3", "scenario": "Standard scenario"}, {"value": "4.63935E-9", "module": "C4", "scenario": "Standard scenario"}, {"value": "-8.6412621E-7", "module": "D", "scenario": "Standard scenario"}, {"name": "referenceToUnitGroupDataSet", "value": {"shortDescription": [{"value": "Disease incidence", "lang": "en"}], "type": "unit group data set", "refObjectId": "3883559b-648f-4afc-8ba2-0bd24f3affa3", "version": "00.00.003", "uri": "../unitgroups/3883559b-648f-4afc-8ba2-0bd24f3affa3.xml"}}]}}, {"referenceToLCIAMethodDataSet": {"shortDescription": [{"value": "Photochemical Ozone Creation Potential (POCP)", "lang": "en"}, {"value": "Bildungspotenzial für troposphärisches Ozon (POCP)", "lang": "de"}], "type": "LCIA method data set", "refObjectId": "b5c610fe-def3-11e6-bf01-fe55135034f3", "version": "02.00.015", "uri": "../lciamethods/b5c610fe-def3-11e6-bf01-fe55135034f3.xml"}, "meanAmount": 0.0, "other": {"anies": [{"value": "0.15672273634382", "module": "A1", "scenario": "Standard scenario"}, {"value": "0.00423876965832", "module": "A2", "scenario": "Standard scenario"}, {"value": "0.00946557184484", "module": "A3", "scenario": "Standard scenario"}, {"value": "0.17042707784698002", "module": "A1-A3", "scenario": "Standard scenario"}, {"value": "0.00139344672751", "module": "A5", "scenario": "Standard scenario"}, {"value": "0.00187761539045", "module": "C1", "scenario": "Standard scenario"}, {"value": "0.00194612161309", "module": "C2", "scenario": "Standard scenario"}, {"value": "0.02799936125", "module": "C3", "scenario": "Standard scenario"}, {"value": "3.0561742E-4", "module": "C4", "scenario": "Standard scenario"}, {"value": "-0.08004355426199", "module": "D", "scenario": "Standard scenario"}, {"name": "referenceToUnitGroupDataSet", "value": {"shortDescription": [{"value": "kg NMVOC-eq.", "lang": "en"}], "type": "unit group data set", "refObjectId": "d27c25f8-fbc1-44c6-b47b-4adbae4199c6", "version": "00.00.003", "uri": "../unitgroups/d27c25f8-fbc1-44c6-b47b-4adbae4199c6.xml"}}]}}, {"referenceToLCIAMethodDataSet": {"shortDescription": [{"value": "Potential Soil quality index (SQP)", "lang": "en"}, {"value": "Potenzieller Bodenqualitätsindex (SQP)", "lang": "de"}], "type": "LCIA method data set", "refObjectId": "b2ad6890-c78d-11e6-9d9d-cec0c932ce01", "version": "01.00.011", "uri": "../lciamethods/b2ad6890-c78d-11e6-9d9d-cec0c932ce01.xml"}, "meanAmount": 0.0, "other": {"anies": [{"value": "181.07963779438", "module": "A1", "scenario": "Standard scenario"}, {"value": "8.61834868623425", "module": "A2", "scenario": "Standard scenario"}, {"value": "562.633279817882", "module": "A3", "scenario": "Standard scenario"}, {"value": "752.3312662984963", "module": "A1-A3", "scenario": "Standard scenario"}, {"value": "0.92995225848549", "module": "A5", "scenario": "Standard scenario"}, {"value": "0.2367640625694", "module": "C1", "scenario": "Standard scenario"}, {"value": "3.95689221152073", "module": "C2", "scenario": "Standard scenario"}, {"value": "67.1248257799999", "module": "C3", "scenario": "Standard scenario"}, {"value": "1.5788200398", "module": "C4", "scenario": "Standard scenario"}, {"value": "-198.457105003421", "module": "D", "scenario": "Standard scenario"}, {"name": "referenceToUnitGroupDataSet", "value": {"shortDescription": [{"value": "dimensionless", "lang": "en"}], "type": "unit group data set", "refObjectId": "f130951c-e67f-4f7f-8dd4-665de3974e18", "version": "00.00.004", "uri": "../unitgroups/f130951c-e67f-4f7f-8dd4-665de3974e18.xml"}}]}}, {"referenceToLCIAMethodDataSet": {"shortDescription": [{"value": "Water (user) deprivation potential (WDP)", "lang": "en"}, {"value": "Wasser-Entzugspotenzial (Benutzer) (WDP)", "lang": "de"}], "type": "LCIA method data set", "refObjectId": "b2ad66ce-c78d-11e6-9d9d-cec0c932ce01", "version": "03.00.015", "uri": "../lciamethods/b2ad66ce-c78d-11e6-9d9d-cec0c932ce01.xml"}, "meanAmount": 0.0, "other": {"anies": [{"value": "8.44961896202396", "module": "A1", "scenario": "Standard scenario"}, {"value": "0.03555387052999", "module": "A2", "scenario": "Standard scenario"}, {"value": "0.40643313205888", "module": "A3", "scenario": "Standard scenario"}, {"value": "8.891605964612829", "module": "A1-A3", "scenario": "Standard scenario"}, {"value": "0.01378968806429", "module": "A5", "scenario": "Standard scenario"}, {"value": "0.00248597584215", "module": "C1", "scenario": "Standard scenario"}, {"value": "0.01632364139713", "module": "C2", "scenario": "Standard scenario"}, {"value": "3.07002627125", "module": "C3", "scenario": "Standard scenario"}, {"value": "0.0286966808", "module": "C4", "scenario": "Standard scenario"}, {"value": "-2.49074022211773", "module": "D", "scenario": "Standard scenario"}, {"name": "referenceToUnitGroupDataSet", "value": {"shortDescription": [{"value": "m3 world eq. deprived", "lang": "en"}], "type": "unit group data set", "refObjectId": "6ae2df01-888e-46c8-b17d-49fa3869b476", "version": "00.00.003", "uri": "../unitgroups/6ae2df01-888e-46c8-b17d-49fa3869b476.xml"}}]}}]}, "otherAttributes": {"{http://www.indata.network/EPD/2019}epd-version": "1.2"}, "version": "1.1"}