{"processInformation": {"dataSetInformation": {"UUID": "1fe33dfb-6ca5-4eed-88b0-73e2e0870674", "name": {"baseName": [{"value": "HIT-RE 500 V4", "lang": "en"}, {"value": "HIT-RE 500 V4", "lang": "de"}], "functionalUnitFlowProperties": [{"lang": "en"}]}, "classificationInformation": {"classification": [{"class": [{"value": "Mineralische Baustoffe", "level": 0, "classId": "1"}, {"value": "Mörtel und Beton", "level": 1, "classId": "1.4"}, {"value": "Kleber und Klebemörtel", "level": 2, "classId": "1.4.05"}], "name": "OEKOBAU.DAT"}, {"class": [{"value": "02 Building products", "level": 0}, {"value": "Construction adhesives and coatings", "level": 1}, {"value": "Reaction resin products", "level": 2}], "name": "IBUCategories"}]}, "generalComment": [{"lang": "en"}]}, "quantitativeReference": {"referenceToReferenceFlow": [0]}, "time": {"referenceYear": 2022, "dataSetValidUntil": 2027, "other": {"anies": [{"name": "publicationDateOfEPD", "value": 1655769600000}]}}, "geography": {"locationOfOperationSupplyOrProduction": {"location": "DE"}}, "technology": {"technologyDescriptionAndIncludedProcesses": [{"value": "All raw materials are sourced from Europe. The transport is exclusively by truck. Chemical mortars are usually two-component systems consisting of a binder and a hardener. The production of chemical mortars consists of a mixing process and a filling process of the respective single components (binder and hardener) and their subsequent union to a two-component system (container). Here as well process control technology is used to weigh and mix solid and liquid compounds according to specification. In the next step both well-mixed components run through an automized filling line in which each of the processed masses is filled into a tubular foil bag. Finally the single components are united in one container. The two-pack foil bags are packed into cardboard boxes and then finally shipped. The manufacturing plant of HIT-RE 500 V4, Hilti GmbH Industriegesellschaft für Befestigungstechnik, Hiltistr. 6, 86916 Kaufering, Germany, is certified according to ISO 9001. The guideline defines international standards for quality and process management. The following flowcharts illustrate the underlying production process Illustration: Production process of the reaction resin mixture Illustration: Production process of the packaging \nDeclared unit: \nThe declared product is a HILTI injection mortar HIT-RE 500 V4. The declared unit refers to one kilogram of reaction resin product in the required mixing ratio of the two components. The packaging of 0,151 kg/kg of product is also included in the calculation. The following table shows the data of the declared unit.", "lang": "en"}, {"value": "Alle Rohstoffe werden aus Europa bezogen. Der Transport erfolgt ausschließlich per LKW. Chemiemörtel sind in der Regel Zweikomponentensysteme, die aus einem Bindemittel und einem Härter bestehen. \n\n\nDie Herstellung von Chemiemörteln besteht aus einem Mischprozess und einem Abfüllprozess der jeweiligen Einzelkomponenten (Bindemittel und Härter) und deren anschließender Vereinigung zu einem Zweikomponentensystem (Gebinde). Auch hier kommt Prozessleittechnik zum Einsatz, um feste und flüssige Mischungen entsprechend der Spezifikation abzuwiegen und zu mischen. Im nächsten Schritt durchlaufen die beiden gut vermischten Komponenten eine automatisierte Abfüllanlage, in der jede der verarbeiteten Massen in einen Folienschlauchbeutel gefüllt wird. Abschließend werden die einzelnen Komponenten in einem Behälter vereinigt. Die Zweier-Folienbeutel werden in Kartons verpackt und schließlich verschickt. Die Produktionsstätte des HIT-RE 500 V4, die Hilti GmbH Industriegesellschaft für Befestigungstechnik, Hiltistr. 6, 86916 Kaufering, Deutschland, ist nach ISO 9001 zertifiziert. Die Richtlinie definiert internationale Standards für Qualitäts- und Prozessmanagement.  \n\nDie folgenden Flussdiagramme veranschaulichen den zugrunde liegenden Produktionsprozess\n\nAbbildung: Herstellungsprozess der Reaktionsharzmischung\n\n\nAbbildung: Herstellungsprozess der Verpackung \n", "lang": "de"}], "technologicalApplicability": [{"value": "Hilti HIT-RE 500 V4 serves for safely securing of threaded rods and post-installed rebar connections in cracked and uncracked concrete C20/25 to C50/60. HIT-RE 500 V4 is ETA and ICC approved for seismic C1 and C2 category for anchoring and C1 category for rebar. \n\n\nHilti HIT-RE-500 V4 is a component of the Hilti SAFEset concept. Hilti SAFEset is an approved system which makes anchor installation an easier, safer and faster process. It significantly improves the robustness of fastening and dramatically reduces the possibilities of error during installation. As part of SAFEset HIT-RE 500 V4 can be installed with approved Hilti Hollow Drill bits and vacuum cleaners that drill and clean the hole in one step for virtually dust-free installation. The use of Hilti HDE-22 dispenser with Volume Calculator app leads to no under or over fill, reducing underfilling related risks and minimizing mortar wastage.", "lang": "en"}, {"value": "Hilti HIT-RE 500 V4 dient zur sicheren Befestigung von Gewindestangen und nachträglich eingebauten Bewehrungsanschlüssen in gerissenem und ungerissenem Beton C20/25 bis C50/60. HIT-RE 500 V4 ist ETA- und ICC-zugelassen für die seismische Kategorie C1 und C2 für Verankerungen und die Kategorie C1 für Bewehrungsstäbe.\n\n \n\nHilti HIT-RE-500 V4 ist eine Komponente des Hilti SAFEset Konzepts. Hilti SAFEset ist ein bewährtes System, das die Ankerinstallation einfacher, sicherer und schneller macht. Es verbessert die Robustheit der Befestigung erheblich und reduziert die Fehlermöglichkeiten bei der Installation drastisch. Als Teil von SAFEset kann der HIT-RE 500 V4 mit zugelassenen Hilti Hohlbohrern und Staubsaugern installiert werden, die das Loch in einem Schritt bohren und reinigen und so eine nahezu staubfreie Installation ermöglichen. Die Verwendung des Hilti HDE-22 Dispensers mit Volumenberechnungs-App führt zu keiner Unter- oder Überfüllung, wodurch die Risiken einer Unterfüllung reduziert und Mörtelverluste minimiert werden.", "lang": "de"}]}}, "modellingAndValidation": {"LCIMethodAndAllocation": {"typeOfDataSet": "EPD", "referenceToLCAMethodDetails": [{"shortDescription": [{"value": "Reaction resin products.pdf", "lang": "en"}], "type": "source data set", "refObjectId": "3c185a17-4d04-4aff-a14e-1f13a12c3b6f"}], "other": {"anies": [{"name": "subType", "value": "specific dataset"}]}}, "dataSourcesTreatmentAndRepresentativeness": {"referenceToDataSource": [{"shortDescription": [{"value": "ecoinvent database (all versions)", "lang": "en"}], "type": "source data set", "refObjectId": "b497a91f-e14b-4b69-8f28-f50eb1576766"}, {"shortDescription": [{"value": "ecoinvent 3.8 database", "lang": "en"}], "type": "source data set", "refObjectId": "0f4c65c0-6210-450f-b886-82bf8dd5ace9"}], "useAdviceForDataSet": [{"value": "Scope: \nThis document refers to the injectable mortar HIT-RE 500 V4 with its packaging. For the compilation of the life cycle assessment, specific data were collected from the factory in Kaufering, Germany, of the HILTI AG. Data from the year 2020 are used, which correspond to the annual average.\n\n\nThe owner of the declaration shall be liable for the underlying information and evidence; the IBU shall not be liable with respect to manufacturer information, life cycle assessment data and evidences. The EPD was created according to the specifications of EN 15804+A2. In the following, the standard will be simplified as EN 15804. \nSystem boundary: \nThe type of the EPD is cradle to grave. The following information modules are defined as system boundaries in this study: \n\n\nA1 – Raw material supply:  \n\nProduction and packaging of the raw materials to be supplied to the manufacturer. All processes are included from cradle to gate. \n\nA2 – Transport (to manufacturing site):  \n\nTransportation of all the raw materials and their packaging between their production site and the manufacturing site, for all transport modes (sea, road).  \n\nA3 – Manufacturing:  \n\nProduction, supply and use of energy sources at the manufacturing sites (electricity, biomass and natural gas). Green electricity  from wind turbines is considered for the whole manufacturing process. \n\nProduction and transport of production losses, final product packaging and other inputs.  \n\nEnd-of-life of production waste (hazardous, non-hazardous and recyclable), production losses and raw material packaging,  including waste and losses transportation, processing and disposal. \n\nA4 – Transport (to construction site) \n\nTransportation of packaged products from the manufacturing site to the construction site, including potential in-betweens (retailer, workshop, etc.). \n\nA5 – Installation-Construction \n\nElectricity consumption for drilling and injecting (in case of injection with electrical dispenser). \n\nProduction of the construction losses. \n\nProvision and end-of-life of tools and accessories for injectable mortars (manual or electrical dispenser with or without battery and with cartridge holder). \n\nEnd-of-life of hazardous construction losses and packaging (uncured mortar and soiled packaging) and non-hazardous construction losses (cured mortar and unsoiled packaging): including waste transportation, processing and disposal. \n\nC1 – Deconstruction/demolition \n\nDiesel for building demolition.  \n\nC2 – Transport (to waste processing) \n\nTransportation to waste processing facility. \n\nC4– Waste disposal  \n\nTreatment and disposal of plastic to sanitary landfill. \n\n\nFor the environmental impact, the use of green electricity (stage A3) was calculated taking into account the residual electricity mix for the remaining electricity. The proportion of the electricity demand covered by green electricity in the total electricity demand is 100%.", "lang": "en"}], "other": {"anies": [{"name": "referenceToOriginalEPD", "value": {"shortDescription": {"value": "HIT-RE 500 V4.pdf", "defaultValue": "HIT-RE 500 V4.pdf", "lstrings": [{"lang": "en", "value": "HIT-RE 500 V4.pdf"}]}, "type": "source data set", "uuid": {"uuid": "8d63ef24-a533-4762-9ec1-24e16020934f"}, "refObjectId": "8d63ef24-a533-4762-9ec1-24e16020934f", "resourceURLs": ["https://oekobaudat.de/OEKOBAU.DAT/resource/sources/8d63ef24-a533-4762-9ec1-24e16020934f/HIT-RE_500_V4_18984.pdf?version=00.02.000"]}}]}}, "validation": {"review": [{"referenceToNameOfReviewerAndInstitution": [{"shortDescription": [{"value": "Institut Bauen und Umwelt e. V.", "lang": "en"}], "type": "contact data set", "refObjectId": "d111dbec-b024-4be5-86c5-752d6eb2cf95", "uri": "../contacts/d111dbec-b024-4be5-86c5-752d6eb2cf95.xml"}], "type": "Accredited third party review"}]}, "complianceDeclarations": {"compliance": [{"referenceToComplianceSystem": {"shortDescription": [{"value": "DIN EN 15804+A2", "lang": "en"}], "type": "source data set", "refObjectId": "c0016b33-8cf7-415c-ac6e-deba0d21440d", "uri": "../sources/c0016b33-8cf7-415c-ac6e-deba0d21440d.xml"}}, {"referenceToComplianceSystem": {"shortDescription": [{"value": "ISO 14025", "lang": "en"}], "type": "source data set", "refObjectId": "4f2eb655-6e44-4874-a95a-e28f5442cd4d", "uri": "../sources/4f2eb655-6e44-4874-a95a-e28f5442cd4d.xml"}}]}}, "administrativeInformation": {"commissionerAndGoal": {"referenceToCommissioner": [{"shortDescription": [{"value": "Hilti Aktiengesellschaft", "lang": "en"}], "type": "contact data set", "refObjectId": "71be6bd4-8792-49c8-bedb-37bd69a50203", "uri": "../contacts/71be6bd4-8792-49c8-bedb-37bd69a50203.xml"}]}, "dataGenerator": {"referenceToPersonOrEntityGeneratingTheDataSet": [{"shortDescription": [{"value": "ESTEANA", "lang": "en"}], "type": "contact data set", "refObjectId": "e24eb42c-f166-42f4-bfad-5b891ee705ca", "uri": "../contacts/e24eb42c-f166-42f4-bfad-5b891ee705ca.xml"}]}, "dataEntryBy": {"timeStamp": 1655800186367, "referenceToDataSetFormat": [{"shortDescription": [{"value": "ILCD Format", "lang": "en"}], "type": "source data set", "refObjectId": "a97a0155-0234-4b87-b4ce-a45da52f2a40", "uri": "../sources/a97a0155-0234-4b87-b4ce-a45da52f2a40.xml"}, {"shortDescription": [{"value": "EPD-Datenformaterweiterungen v1.2", "lang": "de"}, {"value": "EPD Data Format Extensions v1.2", "lang": "en"}], "type": "source data set", "refObjectId": "a29449fd-aa2f-4de8-b5d7-4b06b43c6fde", "uri": "../sources/a29449fd-aa2f-4de8-b5d7-4b06b43c6fde.xml"}]}, "publicationAndOwnership": {"dataSetVersion": "00.03.000", "referenceToRegistrationAuthority": {"shortDescription": [{"value": "Institut Bauen und Umwelt e. V.", "lang": "en"}], "type": "contact data set", "refObjectId": "d111dbec-b024-4be5-86c5-752d6eb2cf95", "uri": "../contacts/d111dbec-b024-4be5-86c5-752d6eb2cf95.xml"}, "registrationNumber": "EPD-HIL-20220125-IBA1-EN", "referenceToOwnershipOfDataSet": {"shortDescription": [{"value": "Hilti Aktiengesellschaft", "lang": "en"}], "type": "contact data set", "refObjectId": "71be6bd4-8792-49c8-bedb-37bd69a50203", "uri": "../contacts/71be6bd4-8792-49c8-bedb-37bd69a50203.xml"}, "copyright": true, "licenseType": "Free of charge for all users and uses", "accessRestrictions": [{"value": "None", "lang": "en"}], "other": {"anies": [{"name": "referenceToPublisher", "value": {"shortDescription": [{"value": "Institut Bauen und Umwelt e. V.", "lang": "en"}], "type": "contact data set", "refObjectId": "d111dbec-b024-4be5-86c5-752d6eb2cf95", "uri": "../contacts/d111dbec-b024-4be5-86c5-752d6eb2cf95.xml"}}]}}}, "exchanges": {"exchange": [{"dataSetInternalID": 0, "referenceToFlowDataSet": {"shortDescription": [{"value": "HIT-RE 500 V4 (HIT-RE 500 V4)", "lang": "en"}], "type": "flow data set", "refObjectId": "535ab207-97d8-e9e3-43dc-602d3be42d91", "uri": "../flows/535ab207-97d8-e9e3-43dc-602d3be42d91.xml"}, "meanAmount": 1.0, "referencesToDataSource": {}, "referenceFlow": true, "resolvedFlowVersion": "00.03.000", "resultingflowAmount": 1.0, "flowProperties": [{"name": [{"lang": "en", "value": "Mass"}, {"lang": "de", "value": "Masse"}], "uuid": "93a60a56-a3c8-11da-a746-0800200b9a66", "referenceFlowProperty": true, "meanValue": 1.0, "referenceUnit": "kg", "unitGroupUUID": "ad38d542-3fe9-439d-9b95-2f5f7752acaf"}], "materialProperties": [{"name": "gross density", "value": "1420.0", "unit": "kg/m^3", "unitDescription": "kilograms per cubic metre"}], "typeOfFlow": "Product flow", "classification": {"classHierarchy": "Mineralische Baustoffe / Mörtel und Beton / Kleber und Klebemörtel", "name": "OEKOBAU.DAT"}}, {"dataSetInternalID": 1, "referenceToFlowDataSet": {"shortDescription": [{"value": "Renewable primary energy as energy carrier (PERE)", "lang": "en"}, {"value": "Erneuerbare Primärenergie als Energieträger (PERE)", "lang": "de"}], "type": "flow data set", "refObjectId": "20f32be5-0398-4288-9b6d-accddd195317", "uri": "../flows/20f32be5-0398-4288-9b6d-accddd195317.xml"}, "exchange direction": "INPUT", "other": {"anies": [{"name": "referenceToUnitGroupDataSet", "value": {"shortDescription": [{"value": "MJ", "lang": "en"}], "type": "unit group data set", "refObjectId": "93a60a57-a3c8-11da-a746-0800200c9a66", "uri": "../unitgroups/93a60a57-a3c8-11da-a746-0800200c9a66.xml"}}, {"value": "13.6023153917605", "module": "A1"}, {"value": "0.0106692308435703", "module": "A2"}, {"value": "0.456381922987196", "module": "A3"}, {"value": "0.0154561523069468", "module": "A4"}, {"value": "1.06586152815005", "module": "A5"}, {"value": "0.000308913822874431", "module": "C1"}, {"value": "0.00104320478671329", "module": "C2"}, {"value": "0", "module": "C3"}, {"value": "0.0117252398300413", "module": "C4"}, {"value": "0", "module": "D"}]}, "resolvedFlowVersion": "38.00.000", "flowProperties": [], "typeOfFlow": "Other flow", "classification": {"classHierarchy": "Quantities", "name": "GaBiCategories"}}, {"dataSetInternalID": 2, "referenceToFlowDataSet": {"shortDescription": [{"value": "Renewable primary energy resources as material utilization (PERM)", "lang": "en"}, {"value": "Erneuerbare Primärenergie zur stofflichen Nutzung (PERM)", "lang": "de"}], "type": "flow data set", "refObjectId": "fb3ec0de-548d-4508-aea5-00b73bf6f702", "uri": "../flows/fb3ec0de-548d-4508-aea5-00b73bf6f702.xml"}, "exchange direction": "INPUT", "other": {"anies": [{"name": "referenceToUnitGroupDataSet", "value": {"shortDescription": [{"value": "MJ", "lang": "en"}], "type": "unit group data set", "refObjectId": "93a60a57-a3c8-11da-a746-0800200c9a66", "uri": "../unitgroups/93a60a57-a3c8-11da-a746-0800200c9a66.xml"}}, {"value": "0", "module": "A1"}, {"value": "0", "module": "A2"}, {"value": "0.681015551686974", "module": "A3"}, {"value": "0", "module": "A4"}, {"value": "0.0476710886180882", "module": "A5"}, {"value": "0", "module": "C1"}, {"value": "0", "module": "C2"}, {"value": "0", "module": "C3"}, {"value": "0", "module": "C4"}, {"value": "0", "module": "D"}]}, "resolvedFlowVersion": "38.00.000", "flowProperties": [], "typeOfFlow": "Other flow", "classification": {"classHierarchy": "Quantities", "name": "GaBiCategories"}}, {"dataSetInternalID": 3, "referenceToFlowDataSet": {"shortDescription": [{"value": "Total use of renewable primary energy resources (PERT)", "lang": "en"}, {"value": "Total erneuerbare Primärenergie (PERT)", "lang": "de"}], "type": "flow data set", "refObjectId": "53f97275-fa8a-4cdd-9024-65936002acd0", "uri": "../flows/53f97275-fa8a-4cdd-9024-65936002acd0.xml"}, "exchange direction": "INPUT", "other": {"anies": [{"name": "referenceToUnitGroupDataSet", "value": {"shortDescription": [{"value": "MJ", "lang": "en"}], "type": "unit group data set", "refObjectId": "93a60a57-a3c8-11da-a746-0800200c9a66", "uri": "../unitgroups/93a60a57-a3c8-11da-a746-0800200c9a66.xml"}}, {"value": "13.6023153917605", "module": "A1"}, {"value": "0.0106692308435703", "module": "A2"}, {"value": "1.13739747467417", "module": "A3"}, {"value": "0.0154561523069468", "module": "A4"}, {"value": "1.11353261676813", "module": "A5"}, {"value": "0.000308913822874431", "module": "C1"}, {"value": "0.00104320478671329", "module": "C2"}, {"value": "0", "module": "C3"}, {"value": "0.0117252398300413", "module": "C4"}, {"value": "0", "module": "D"}]}, "resolvedFlowVersion": "38.00.000", "flowProperties": [], "typeOfFlow": "Other flow", "classification": {"classHierarchy": "Quantities / Environmental quantities / EPD EN 15804 / LCI indicators", "name": "GaBiCategories"}}, {"dataSetInternalID": 4, "referenceToFlowDataSet": {"shortDescription": [{"value": "Non renewable primary energy as energy carrier (PENRE)", "lang": "en"}, {"value": "Nicht-erneuerbare Primärenergie als Energieträger (PENRE)", "lang": "de"}], "type": "flow data set", "refObjectId": "ac857178-2b45-46ec-892a-a9a4332f0372", "uri": "../flows/ac857178-2b45-46ec-892a-a9a4332f0372.xml"}, "exchange direction": "INPUT", "other": {"anies": [{"name": "referenceToUnitGroupDataSet", "value": {"shortDescription": [{"value": "MJ", "lang": "en"}], "type": "unit group data set", "refObjectId": "93a60a57-a3c8-11da-a746-0800200c9a66", "uri": "../unitgroups/93a60a57-a3c8-11da-a746-0800200c9a66.xml"}}, {"value": "37.7391016889329", "module": "A1"}, {"value": "0.733411479886188", "module": "A2"}, {"value": "5.63647449183168", "module": "A3"}, {"value": "1.06246829813561", "module": "A4"}, {"value": "4.81512599862049", "module": "A5"}, {"value": "0.0540556697322197", "module": "C1"}, {"value": "0.0717107331976816", "module": "C2"}, {"value": "0", "module": "C3"}, {"value": "0.221989077563813", "module": "C4"}, {"value": "0", "module": "D"}]}, "resolvedFlowVersion": "38.00.000", "flowProperties": [], "typeOfFlow": "Other flow", "classification": {"classHierarchy": "Quantities", "name": "GaBiCategories"}}, {"dataSetInternalID": 5, "referenceToFlowDataSet": {"shortDescription": [{"value": "Non renewable primary energy as material utilization (PENRM)", "lang": "en"}, {"value": "Nicht-erneuerbare Primärenergie zur stofflichen Nutzung (PENRM)", "lang": "de"}], "type": "flow data set", "refObjectId": "1421caa0-679d-4bf4-b282-0eb850ccae27", "uri": "../flows/1421caa0-679d-4bf4-b282-0eb850ccae27.xml"}, "exchange direction": "INPUT", "other": {"anies": [{"name": "referenceToUnitGroupDataSet", "value": {"shortDescription": [{"value": "MJ", "lang": "en"}], "type": "unit group data set", "refObjectId": "93a60a57-a3c8-11da-a746-0800200c9a66", "uri": "../unitgroups/93a60a57-a3c8-11da-a746-0800200c9a66.xml"}}, {"value": "20.6893", "module": "A1"}, {"value": "0", "module": "A2"}, {"value": "2.68195962116912", "module": "A3"}, {"value": "0", "module": "A4"}, {"value": "1.67808455058791", "module": "A5"}, {"value": "0", "module": "C1"}, {"value": "0", "module": "C2"}, {"value": "0", "module": "C3"}, {"value": "0", "module": "C4"}, {"value": "0", "module": "D"}]}, "resolvedFlowVersion": "38.00.000", "flowProperties": [], "typeOfFlow": "Other flow", "classification": {"classHierarchy": "Quantities", "name": "GaBiCategories"}}, {"dataSetInternalID": 6, "referenceToFlowDataSet": {"shortDescription": [{"value": "Total use of non renewable primary energy resources (PENRT)", "lang": "en"}, {"value": "Total nicht erneuerbare Primärenergie (PENRT)", "lang": "de"}], "type": "flow data set", "refObjectId": "06159210-646b-4c8d-8583-da9b3b95a6c1", "uri": "../flows/06159210-646b-4c8d-8583-da9b3b95a6c1.xml"}, "exchange direction": "INPUT", "other": {"anies": [{"name": "referenceToUnitGroupDataSet", "value": {"shortDescription": [{"value": "MJ", "lang": "en"}], "type": "unit group data set", "refObjectId": "93a60a57-a3c8-11da-a746-0800200c9a66", "uri": "../unitgroups/93a60a57-a3c8-11da-a746-0800200c9a66.xml"}}, {"value": "58.4284016889329", "module": "A1"}, {"value": "0.733411479886188", "module": "A2"}, {"value": "8.3184341130008", "module": "A3"}, {"value": "1.06246829813561", "module": "A4"}, {"value": "6.49321054920841", "module": "A5"}, {"value": "0.0540556697322197", "module": "C1"}, {"value": "0.0717107331976816", "module": "C2"}, {"value": "0", "module": "C3"}, {"value": "0.221989077563813", "module": "C4"}, {"value": "0", "module": "D"}]}, "resolvedFlowVersion": "38.00.000", "flowProperties": [], "typeOfFlow": "Other flow", "classification": {"classHierarchy": "Quantities / Environmental quantities / EPD EN 15804 / LCI indicators", "name": "GaBiCategories"}}, {"dataSetInternalID": 7, "referenceToFlowDataSet": {"shortDescription": [{"value": "Use of secondary material (SM)", "lang": "en"}, {"value": "Einsatz von Sekundärstoffen (SM)", "lang": "de"}], "type": "flow data set", "refObjectId": "c6a1f35f-2d09-4f54-8dfb-97e502e1ce92", "uri": "../flows/c6a1f35f-2d09-4f54-8dfb-97e502e1ce92.xml"}, "exchange direction": "INPUT", "other": {"anies": [{"name": "referenceToUnitGroupDataSet", "value": {"shortDescription": [{"value": "kg", "lang": "en"}], "type": "unit group data set", "refObjectId": "ad38d542-3fe9-439d-9b95-2f5f7752acaf", "uri": "../unitgroups/ad38d542-3fe9-439d-9b95-2f5f7752acaf.xml"}}, {"value": "0.0173929288823305", "module": "A1"}, {"value": "0.000249646159626837", "module": "A2"}, {"value": "0.0830639569158912", "module": "A3"}, {"value": "0.000361653911384066", "module": "A4"}, {"value": "0.00869864108590671", "module": "A5"}, {"value": "2.11542036926058E-05", "module": "C1"}, {"value": "2.44096385696118E-05", "module": "C2"}, {"value": "0", "module": "C3"}, {"value": "8.41290170820906E-05", "module": "C4"}, {"value": "0", "module": "D"}]}, "resolvedFlowVersion": "38.00.000", "flowProperties": [], "typeOfFlow": "Other flow", "classification": {"classHierarchy": "Quantities / Environmental quantities / EPD EN 15804 / LCI indicators", "name": "GaBiCategories"}}, {"dataSetInternalID": 8, "referenceToFlowDataSet": {"shortDescription": [{"value": "Use of renewable secondary fuels (RSF)", "lang": "en"}, {"value": "Erneuerbare Sekundärbrennstoffe (RSF)", "lang": "de"}], "type": "flow data set", "refObjectId": "64333088-a55f-4aa2-9a31-c10b07816787", "uri": "../flows/64333088-a55f-4aa2-9a31-c10b07816787.xml"}, "exchange direction": "INPUT", "other": {"anies": [{"name": "referenceToUnitGroupDataSet", "value": {"shortDescription": [{"value": "MJ", "lang": "en"}], "type": "unit group data set", "refObjectId": "93a60a57-a3c8-11da-a746-0800200c9a66", "uri": "../unitgroups/93a60a57-a3c8-11da-a746-0800200c9a66.xml"}}, {"value": "0.000329379110355398", "module": "A1"}, {"value": "2.74738962269014E-06", "module": "A2"}, {"value": "0.00671616780673776", "module": "A3"}, {"value": "3.98005002210765E-06", "module": "A4"}, {"value": "0.00052018118215082", "module": "A5"}, {"value": "6.91327733208197E-08", "module": "C1"}, {"value": "2.68631361283553E-07", "module": "C2"}, {"value": "0", "module": "C3"}, {"value": "3.83093443829271E-06", "module": "C4"}, {"value": "0", "module": "D"}]}, "resolvedFlowVersion": "38.00.000", "flowProperties": [], "typeOfFlow": "Other flow", "classification": {"classHierarchy": "Quantities / Environmental quantities / EPD EN 15804 / LCI indicators", "name": "GaBiCategories"}}, {"dataSetInternalID": 9, "referenceToFlowDataSet": {"shortDescription": [{"value": "Use of non renewable secondary fuels (NRSF)", "lang": "en"}, {"value": "Nicht erneuerbare Sekundärbrennstoffe (NRSF)", "lang": "de"}], "type": "flow data set", "refObjectId": "89def144-d39a-4287-b86f-efde453ddcb2", "uri": "../flows/89def144-d39a-4287-b86f-efde453ddcb2.xml"}, "exchange direction": "INPUT", "other": {"anies": [{"name": "referenceToUnitGroupDataSet", "value": {"shortDescription": [{"value": "MJ", "lang": "en"}], "type": "unit group data set", "refObjectId": "93a60a57-a3c8-11da-a746-0800200c9a66", "uri": "../unitgroups/93a60a57-a3c8-11da-a746-0800200c9a66.xml"}}, {"value": "0", "module": "A1"}, {"value": "0", "module": "A2"}, {"value": "0", "module": "A3"}, {"value": "0", "module": "A4"}, {"value": "0", "module": "A5"}, {"value": "0", "module": "C1"}, {"value": "0", "module": "C2"}, {"value": "0", "module": "C3"}, {"value": "0", "module": "C4"}, {"value": "0", "module": "D"}]}, "resolvedFlowVersion": "38.00.000", "flowProperties": [], "typeOfFlow": "Other flow", "classification": {"classHierarchy": "Quantities / Environmental quantities / EPD EN 15804 / LCI indicators", "name": "GaBiCategories"}}, {"dataSetInternalID": 10, "referenceToFlowDataSet": {"shortDescription": [{"value": "Use of net fresh water (FW)", "lang": "en"}, {"value": "Einsatz von Süßwasserressourcen (FW)", "lang": "de"}], "type": "flow data set", "refObjectId": "3cf952c8-f3a4-461d-8c96-96456ca62246", "uri": "../flows/3cf952c8-f3a4-461d-8c96-96456ca62246.xml"}, "exchange direction": "INPUT", "other": {"anies": [{"name": "referenceToUnitGroupDataSet", "value": {"shortDescription": [{"value": "m^3", "lang": "en"}], "type": "unit group data set", "refObjectId": "cd950537-0a98-4044-9ba7-9f9a68d0a504", "uri": "../unitgroups/cd950537-0a98-4044-9ba7-9f9a68d0a504.xml"}}, {"value": "0.130103784208451", "module": "A1"}, {"value": "9.34989648267896E-05", "module": "A2"}, {"value": "0.00566451164547263", "module": "A3"}, {"value": "0.000135448774339306", "module": "A4"}, {"value": "0.0108688122301539", "module": "A5"}, {"value": "3.28244778011065E-06", "module": "C1"}, {"value": "9.1420430479133E-06", "module": "C2"}, {"value": "0", "module": "C3"}, {"value": "0.000291741981689063", "module": "C4"}, {"value": "0", "module": "D"}]}, "resolvedFlowVersion": "38.00.000", "flowProperties": [], "typeOfFlow": "Other flow", "classification": {"classHierarchy": "Quantities / Environmental quantities / EPD EN 15804 / LCI indicators", "name": "GaBiCategories"}}, {"dataSetInternalID": 11, "referenceToFlowDataSet": {"shortDescription": [{"value": "Hazardous waste disposed (HWD)", "lang": "en"}, {"value": "Gefährlicher Abfall zur Deponie (HWD)", "lang": "de"}], "type": "flow data set", "refObjectId": "430f9e0f-59b2-46a0-8e0d-55e0e84948fc", "uri": "../flows/430f9e0f-59b2-46a0-8e0d-55e0e84948fc.xml"}, "exchange direction": "OUTPUT", "other": {"anies": [{"name": "referenceToUnitGroupDataSet", "value": {"shortDescription": [{"value": "kg", "lang": "en"}], "type": "unit group data set", "refObjectId": "ad38d542-3fe9-439d-9b95-2f5f7752acaf", "uri": "../unitgroups/ad38d542-3fe9-439d-9b95-2f5f7752acaf.xml"}}, {"value": "0.292654485070312", "module": "A1"}, {"value": "0.000834217064072368", "module": "A2"}, {"value": "0.0417248369359936", "module": "A3"}, {"value": "0.00120850192374708", "module": "A4"}, {"value": "0.184964619839818", "module": "A5"}, {"value": "7.23264993202179E-05", "module": "C1"}, {"value": "8.15671951575262E-05", "module": "C2"}, {"value": "0", "module": "C3"}, {"value": "0.000346321939029426", "module": "C4"}, {"value": "0", "module": "D"}]}, "resolvedFlowVersion": "38.00.000", "flowProperties": [], "typeOfFlow": "Other flow", "classification": {"classHierarchy": "Quantities / Environmental quantities / EPD EN 15804 / LCI indicators", "name": "GaBiCategories"}}, {"dataSetInternalID": 12, "referenceToFlowDataSet": {"shortDescription": [{"value": "Non hazardous waste disposed (NHWD)", "lang": "en"}, {"value": "Entsorgter nicht gefährlicher Abfall (NHWD)", "lang": "de"}], "type": "flow data set", "refObjectId": "b29ef66b-e286-4afa-949f-62f1a7b4d7fa", "uri": "../flows/b29ef66b-e286-4afa-949f-62f1a7b4d7fa.xml"}, "exchange direction": "OUTPUT", "other": {"anies": [{"name": "referenceToUnitGroupDataSet", "value": {"shortDescription": [{"value": "kg", "lang": "en"}], "type": "unit group data set", "refObjectId": "ad38d542-3fe9-439d-9b95-2f5f7752acaf", "uri": "../unitgroups/ad38d542-3fe9-439d-9b95-2f5f7752acaf.xml"}}, {"value": "4.16922648987737", "module": "A1"}, {"value": "0.0148252473819877", "module": "A2"}, {"value": "0.501636420306532", "module": "A3"}, {"value": "0.0214768322931408", "module": "A4"}, {"value": "0.487112537476845", "module": "A5"}, {"value": "0.000508364614718604", "module": "C1"}, {"value": "0.00144956738305258", "module": "C2"}, {"value": "0", "module": "C3"}, {"value": "1.00326999759673", "module": "C4"}, {"value": "0", "module": "D"}]}, "resolvedFlowVersion": "38.00.000", "flowProperties": [], "typeOfFlow": "Other flow", "classification": {"classHierarchy": "Quantities / Environmental quantities / EPD EN 15804 / LCI indicators", "name": "GaBiCategories"}}, {"dataSetInternalID": 13, "referenceToFlowDataSet": {"shortDescription": [{"value": "Radioactive waste disposed (RWD)", "lang": "en"}, {"value": "Entsorgter radioaktiver Abfall (RWD)", "lang": "de"}], "type": "flow data set", "refObjectId": "3449546e-52ad-4b39-b809-9fb77cea8ff6", "uri": "../flows/3449546e-52ad-4b39-b809-9fb77cea8ff6.xml"}, "exchange direction": "OUTPUT", "other": {"anies": [{"name": "referenceToUnitGroupDataSet", "value": {"shortDescription": [{"value": "kg", "lang": "en"}], "type": "unit group data set", "refObjectId": "ad38d542-3fe9-439d-9b95-2f5f7752acaf", "uri": "../unitgroups/ad38d542-3fe9-439d-9b95-2f5f7752acaf.xml"}}, {"value": "9.56624917162317E-05", "module": "A1"}, {"value": "5.0469099117276E-06", "module": "A2"}, {"value": "1.41361154770761E-05", "module": "A3"}, {"value": "7.31128695393353E-06", "module": "A4"}, {"value": "1.76744460900929E-05", "module": "A5"}, {"value": "3.80503086428119E-07", "module": "C1"}, {"value": "4.93471427811296E-07", "module": "C2"}, {"value": "0", "module": "C3"}, {"value": "1.4732803421208E-06", "module": "C4"}, {"value": "0", "module": "D"}]}, "resolvedFlowVersion": "38.00.000", "flowProperties": [], "typeOfFlow": "Other flow", "classification": {"classHierarchy": "Quantities / Environmental quantities / EPD EN 15804 / LCI indicators", "name": "GaBiCategories"}}, {"dataSetInternalID": 14, "referenceToFlowDataSet": {"shortDescription": [{"value": "Components for re-use (CRU)", "lang": "en"}, {"value": "Komponenten für die Wiederverwendung (CRU)", "lang": "de"}], "type": "flow data set", "refObjectId": "a2b32f97-3fc7-4af2-b209-525bc6426f33", "uri": "../flows/a2b32f97-3fc7-4af2-b209-525bc6426f33.xml"}, "exchange direction": "OUTPUT", "other": {"anies": [{"name": "referenceToUnitGroupDataSet", "value": {"shortDescription": [{"value": "kg", "lang": "en"}], "type": "unit group data set", "refObjectId": "ad38d542-3fe9-439d-9b95-2f5f7752acaf", "uri": "../unitgroups/ad38d542-3fe9-439d-9b95-2f5f7752acaf.xml"}}, {"value": "0", "module": "A1"}, {"value": "0", "module": "A2"}, {"value": "0", "module": "A3"}, {"value": "0", "module": "A4"}, {"value": "0", "module": "A5"}, {"value": "0", "module": "C1"}, {"value": "0", "module": "C2"}, {"value": "0", "module": "C3"}, {"value": "0", "module": "C4"}, {"value": "0", "module": "D"}]}, "resolvedFlowVersion": "38.00.000", "flowProperties": [], "typeOfFlow": "Other flow", "classification": {"classHierarchy": "Quantities / Environmental quantities / EPD EN 15804 / LCI indicators", "name": "GaBiCategories"}}, {"dataSetInternalID": 15, "referenceToFlowDataSet": {"shortDescription": [{"value": "Materials for recycling (MFR)", "lang": "en"}, {"value": "Stoffe zum Recycling (MFR)", "lang": "de"}], "type": "flow data set", "refObjectId": "d7fe48a5-4103-49c8-9aae-b0b5dfdbd6ae", "uri": "../flows/d7fe48a5-4103-49c8-9aae-b0b5dfdbd6ae.xml"}, "exchange direction": "OUTPUT", "other": {"anies": [{"name": "referenceToUnitGroupDataSet", "value": {"shortDescription": [{"value": "kg", "lang": "en"}], "type": "unit group data set", "refObjectId": "ad38d542-3fe9-439d-9b95-2f5f7752acaf", "uri": "../unitgroups/ad38d542-3fe9-439d-9b95-2f5f7752acaf.xml"}}, {"value": "0.00589070081330341", "module": "A1"}, {"value": "2.29852931942256E-06", "module": "A2"}, {"value": "0.051013802423524", "module": "A3"}, {"value": "3.32980134780637E-06", "module": "A4"}, {"value": "0.0935165657415933", "module": "A5"}, {"value": "7.20090936898767E-08", "module": "C1"}, {"value": "2.24743172547202E-07", "module": "C2"}, {"value": "0", "module": "C3"}, {"value": "1.21423300604748E-06", "module": "C4"}, {"value": "0", "module": "D"}]}, "resolvedFlowVersion": "38.00.000", "flowProperties": [], "typeOfFlow": "Other flow", "classification": {"classHierarchy": "Quantities / Environmental quantities / EPD EN 15804 / LCI indicators", "name": "GaBiCategories"}}, {"dataSetInternalID": 16, "referenceToFlowDataSet": {"shortDescription": [{"value": "Materials for energy recovery (MER)", "lang": "en"}, {"value": "Stoffe für die Energierückgewinnung (MER)", "lang": "de"}], "type": "flow data set", "refObjectId": "59a9181c-3aaf-46ee-8b13-2b3723b6e447", "uri": "../flows/59a9181c-3aaf-46ee-8b13-2b3723b6e447.xml"}, "exchange direction": "OUTPUT", "other": {"anies": [{"name": "referenceToUnitGroupDataSet", "value": {"shortDescription": [{"value": "kg", "lang": "en"}], "type": "unit group data set", "refObjectId": "ad38d542-3fe9-439d-9b95-2f5f7752acaf", "uri": "../unitgroups/ad38d542-3fe9-439d-9b95-2f5f7752acaf.xml"}}, {"value": "0.0152418716027612", "module": "A1"}, {"value": "1.84725599171543E-08", "module": "A2"}, {"value": "1.10568400036263E-05", "module": "A3"}, {"value": "2.67605700696596E-08", "module": "A4"}, {"value": "0.0010678277292543", "module": "A5"}, {"value": "1.15247875008429E-09", "module": "C1"}, {"value": "1.80619045655354E-09", "module": "C2"}, {"value": "0", "module": "C3"}, {"value": "5.84731872933728E-09", "module": "C4"}, {"value": "0", "module": "D"}]}, "resolvedFlowVersion": "38.00.000", "flowProperties": [], "typeOfFlow": "Other flow", "classification": {"classHierarchy": "Quantities / Environmental quantities / EPD EN 15804 / LCI indicators", "name": "GaBiCategories"}}, {"dataSetInternalID": 17, "referenceToFlowDataSet": {"shortDescription": [{"value": "Exported electrical energy (EEE)", "lang": "en"}, {"value": "Exportierte elektrische Energie (EEE)", "lang": "de"}], "type": "flow data set", "refObjectId": "4da0c987-2b76-40d6-9e9e-82a017aaaf29", "uri": "../flows/4da0c987-2b76-40d6-9e9e-82a017aaaf29.xml"}, "exchange direction": "OUTPUT", "other": {"anies": [{"name": "referenceToUnitGroupDataSet", "value": {"shortDescription": [{"value": "MJ", "lang": "en"}], "type": "unit group data set", "refObjectId": "93a60a57-a3c8-11da-a746-0800200c9a66", "uri": "../unitgroups/93a60a57-a3c8-11da-a746-0800200c9a66.xml"}}, {"value": "0.0330189777393877", "module": "A1"}, {"value": "0.000159690639056093", "module": "A2"}, {"value": "0.00735403321419298", "module": "A3"}, {"value": "0.000231338404373551", "module": "A4"}, {"value": "0.00381700615352116", "module": "A5"}, {"value": "2.11954112336406E-05", "module": "C1"}, {"value": "1.56140626722885E-05", "module": "C2"}, {"value": "0", "module": "C3"}, {"value": "0.000453303871682149", "module": "C4"}, {"value": "0", "module": "D"}]}, "resolvedFlowVersion": "38.00.000", "flowProperties": [], "typeOfFlow": "Other flow", "classification": {"classHierarchy": "Quantities / Environmental quantities / EPD EN 15804 / LCI indicators", "name": "GaBiCategories"}}, {"dataSetInternalID": 18, "referenceToFlowDataSet": {"shortDescription": [{"value": "Exported thermal energy (EET)", "lang": "en"}, {"value": "Exportierte thermische Energie (EET)", "lang": "de"}], "type": "flow data set", "refObjectId": "98daf38a-7a79-46d3-9a37-2b7bd0955810", "uri": "../flows/98daf38a-7a79-46d3-9a37-2b7bd0955810.xml"}, "exchange direction": "OUTPUT", "other": {"anies": [{"name": "referenceToUnitGroupDataSet", "value": {"shortDescription": [{"value": "MJ", "lang": "en"}], "type": "unit group data set", "refObjectId": "93a60a57-a3c8-11da-a746-0800200c9a66", "uri": "../unitgroups/93a60a57-a3c8-11da-a746-0800200c9a66.xml"}}, {"value": "0.13157939130117", "module": "A1"}, {"value": "0.00066406577569967", "module": "A2"}, {"value": "0.0213176964977652", "module": "A3"}, {"value": "0.000962009532039532", "module": "A4"}, {"value": "0.014225233254693", "module": "A5"}, {"value": "0.00021455956720392", "module": "C1"}, {"value": "6.49303221628061E-05", "module": "C2"}, {"value": "0", "module": "C3"}, {"value": "0.001222807045117", "module": "C4"}, {"value": "0", "module": "D"}]}, "resolvedFlowVersion": "38.00.000", "flowProperties": [], "typeOfFlow": "Other flow", "classification": {"classHierarchy": "Quantities / Environmental quantities / EPD EN 15804 / LCI indicators", "name": "GaBiCategories"}}]}, "LCIAResults": {"LCIAResult": [{"referenceToLCIAMethodDataSet": {"shortDescription": [{"value": "Global Warming Potential total (GWP-total)", "lang": "en"}, {"value": "Globales Erwärmungspotenzial total (GWP-total)", "lang": "de"}], "type": "LCIA method data set", "refObjectId": "6a37f984-a4b3-458a-a20a-64418c145fa2", "uri": "../lciamethods/6a37f984-a4b3-458a-a20a-64418c145fa2.xml"}, "other": {"anies": [{"name": "referenceToUnitGroupDataSet", "value": {"shortDescription": [{"value": "kg CO_(2)-Äq.", "lang": "en"}], "type": "unit group data set", "refObjectId": "1ebf3012-d0db-4de2-aefd-ef30cedb0be1", "uri": "../unitgroups/1ebf3012-d0db-4de2-aefd-ef30cedb0be1.xml"}}, {"value": "3.24969285280096", "module": "A1"}, {"value": "0.049466443924089", "module": "A2"}, {"value": "0.474571898385709", "module": "A3"}, {"value": "0.0716603570195045", "module": "A4"}, {"value": "0.57222567742344", "module": "A5"}, {"value": "0.00402168059972286", "module": "C1"}, {"value": "0.00483667771743755", "module": "C2"}, {"value": "0", "module": "C3"}, {"value": "0.114307348827589", "module": "C4"}, {"value": "0", "module": "D"}]}}, {"referenceToLCIAMethodDataSet": {"shortDescription": [{"value": "Global Warming Potential fossil fuels (GWP-fossil)", "lang": "en"}, {"value": "Globales Erwärmungspotenzial fossil (GWP-fossil)", "lang": "de"}], "type": "LCIA method data set", "refObjectId": "5f635281-343e-44fb-83df-1971b155e6b6", "uri": "../lciamethods/5f635281-343e-44fb-83df-1971b155e6b6.xml"}, "other": {"anies": [{"name": "referenceToUnitGroupDataSet", "value": {"shortDescription": [{"value": "kg CO_(2)-Äq.", "lang": "en"}], "type": "unit group data set", "refObjectId": "1ebf3012-d0db-4de2-aefd-ef30cedb0be1", "uri": "../unitgroups/1ebf3012-d0db-4de2-aefd-ef30cedb0be1.xml"}}, {"value": "3.10281327369234", "module": "A1"}, {"value": "0.0492755719259797", "module": "A2"}, {"value": "0.443305347937552", "module": "A3"}, {"value": "0.0713838472394498", "module": "A4"}, {"value": "0.558425874934043", "module": "A5"}, {"value": "0.00401763318869546", "module": "C1"}, {"value": "0.00481801483676728", "module": "C2"}, {"value": "0", "module": "C3"}, {"value": "0.114019717879823", "module": "C4"}, {"value": "0", "module": "D"}]}}, {"referenceToLCIAMethodDataSet": {"shortDescription": [{"value": "Global Warming Potential biogenic (GWP-biogenic)", "lang": "en"}, {"value": "Globales Erwärmungspotenzial biogen (GWP-biogenic)", "lang": "de"}], "type": "LCIA method data set", "refObjectId": "2356e1ab-0185-4db5-86e5-16de51c7485c", "uri": "../lciamethods/2356e1ab-0185-4db5-86e5-16de51c7485c.xml"}, "other": {"anies": [{"name": "referenceToUnitGroupDataSet", "value": {"shortDescription": [{"value": "kg CO_(2)-Äq.", "lang": "en"}], "type": "unit group data set", "refObjectId": "1ebf3012-d0db-4de2-aefd-ef30cedb0be1", "uri": "../unitgroups/1ebf3012-d0db-4de2-aefd-ef30cedb0be1.xml"}}, {"value": "0.0404383733414173", "module": "A1"}, {"value": "0.000171174815998529", "module": "A2"}, {"value": "0.0303154864388604", "module": "A3"}, {"value": "0.000247975141411553", "module": "A4"}, {"value": "0.00618388953190477", "module": "A5"}, {"value": "3.64738200621849E-06", "module": "C1"}, {"value": "1.67369503980735E-05", "module": "C2"}, {"value": "0", "module": "C3"}, {"value": "0.000285483172843197", "module": "C4"}, {"value": "0", "module": "D"}]}}, {"referenceToLCIAMethodDataSet": {"shortDescription": [{"value": "Global Warming Potential luluc (GWP-luluc)", "lang": "en"}, {"value": "Globales Erwärmungspotenzial luluc (GWP-luluc)", "lang": "de"}], "type": "LCIA method data set", "refObjectId": "4331bbdb-978a-490d-8707-eeb047f01a55", "uri": "../lciamethods/4331bbdb-978a-490d-8707-eeb047f01a55.xml"}, "other": {"anies": [{"name": "referenceToUnitGroupDataSet", "value": {"shortDescription": [{"value": "kg CO_(2)-Äq.", "lang": "en"}], "type": "unit group data set", "refObjectId": "1ebf3012-d0db-4de2-aefd-ef30cedb0be1", "uri": "../unitgroups/1ebf3012-d0db-4de2-aefd-ef30cedb0be1.xml"}}, {"value": "0.106441205767203", "module": "A1"}, {"value": "1.96971821107693E-05", "module": "A2"}, {"value": "0.000951064009296076", "module": "A3"}, {"value": "2.85346386431581E-05", "module": "A4"}, {"value": "0.00761591295749235", "module": "A5"}, {"value": "4.00029021176389E-07", "module": "C1"}, {"value": "1.9259302721996E-06", "module": "C2"}, {"value": "0", "module": "C3"}, {"value": "2.1477749227705E-06", "module": "C4"}, {"value": "0", "module": "D"}]}}, {"referenceToLCIAMethodDataSet": {"shortDescription": [{"value": "Depletion potential of the stratospheric ozone layer (ODP)", "lang": "en"}, {"value": "Abbau Potential der stratosphärischen Ozonschicht (ODP)", "lang": "de"}], "type": "LCIA method data set", "refObjectId": "b5c629d6-def3-11e6-bf01-fe55135034f3", "uri": "../lciamethods/b5c629d6-def3-11e6-bf01-fe55135034f3.xml"}, "other": {"anies": [{"name": "referenceToUnitGroupDataSet", "value": {"shortDescription": [{"value": "kg CFC11-Äq.", "lang": "en"}], "type": "unit group data set", "refObjectId": "d9e957c9-7309-4474-bf3a-7777df6c4e5b", "uri": "../unitgroups/d9e957c9-7309-4474-bf3a-7777df6c4e5b.xml"}}, {"value": "4.12687739442879E-07", "module": "A1"}, {"value": "1.14171485524442E-08", "module": "A2"}, {"value": "5.65794306674928E-08", "module": "A3"}, {"value": "1.65396352862643E-08", "module": "A4"}, {"value": "6.98194156524131E-08", "module": "A5"}, {"value": "8.58748046526841E-10", "module": "C1"}, {"value": "1.11633389465035E-09", "module": "C2"}, {"value": "0", "module": "C3"}, {"value": "3.102127676718E-09", "module": "C4"}, {"value": "0", "module": "D"}]}}, {"referenceToLCIAMethodDataSet": {"shortDescription": [{"value": "Acidification potential of land and water (AP)", "lang": "en"}, {"value": "Versauerungspotenzial von Boden und Wasser (AP)", "lang": "de"}], "type": "LCIA method data set", "refObjectId": "b5c611c6-def3-11e6-bf01-fe55135034f3", "uri": "../lciamethods/b5c611c6-def3-11e6-bf01-fe55135034f3.xml"}, "other": {"anies": [{"name": "referenceToUnitGroupDataSet", "value": {"shortDescription": [{"value": "mol H^(+)-Äq.", "lang": "en"}], "type": "unit group data set", "refObjectId": "42e089ac-92bf-4bf2-8ca1-5fc40d18f2ed", "uri": "../unitgroups/42e089ac-92bf-4bf2-8ca1-5fc40d18f2ed.xml"}}, {"value": "0.0166638321133941", "module": "A1"}, {"value": "0.000139973926554624", "module": "A2"}, {"value": "0.00204044803624849", "module": "A3"}, {"value": "0.000202775472716801", "module": "A4"}, {"value": "0.00234303143617375", "module": "A5"}, {"value": "4.17393002642394E-05", "module": "C1"}, {"value": "1.36862227781711E-05", "module": "C2"}, {"value": "0", "module": "C3"}, {"value": "7.62995469148324E-05", "module": "C4"}, {"value": "0", "module": "D"}]}}, {"referenceToLCIAMethodDataSet": {"shortDescription": [{"value": "Eutrophication potential aquatic freshwater (EP-freshwater)", "lang": "en"}, {"value": "Eutrophierungspotenzial Süßwasser (EP-freshwater)", "lang": "de"}], "type": "LCIA method data set", "refObjectId": "b53ec18f-7377-4ad3-86eb-cc3f4f276b2b", "uri": "../lciamethods/b53ec18f-7377-4ad3-86eb-cc3f4f276b2b.xml"}, "other": {"anies": [{"name": "referenceToUnitGroupDataSet", "value": {"shortDescription": [{"value": "kg PO_(4)-Äq.", "lang": "en"}], "type": "unit group data set", "refObjectId": "0429039d-a61d-4590-ba67-aa4a20a810a1", "uri": "../unitgroups/0429039d-a61d-4590-ba67-aa4a20a810a1.xml"}}, {"value": "0.000991181485533868", "module": "A1"}, {"value": "3.37013053419532E-06", "module": "A2"}, {"value": "0.000135901700609896", "module": "A3"}, {"value": "4.88219362712595E-06", "module": "A4"}, {"value": "0.000170643309670044", "module": "A5"}, {"value": "1.26606419512521E-07", "module": "C1"}, {"value": "3.29521064514213E-07", "module": "C2"}, {"value": "0", "module": "C3"}, {"value": "8.57808383354582E-07", "module": "C4"}, {"value": "0", "module": "D"}]}}, {"referenceToLCIAMethodDataSet": {"shortDescription": [{"value": "Eutrophication potential aquatic marine (EP-marine)", "lang": "en"}, {"value": "Eutrophierungspotenzial Salzwasser (EP-marine)", "lang": "de"}], "type": "LCIA method data set", "refObjectId": "b5c619fa-def3-11e6-bf01-fe55135034f3", "uri": "../lciamethods/b5c619fa-def3-11e6-bf01-fe55135034f3.xml"}, "other": {"anies": [{"name": "referenceToUnitGroupDataSet", "value": {"shortDescription": [{"value": "kg N-Äq.", "lang": "en"}], "type": "unit group data set", "refObjectId": "d05bb823-ecdf-4686-8c40-bf1d9257859f", "uri": "../unitgroups/d05bb823-ecdf-4686-8c40-bf1d9257859f.xml"}}, {"value": "0.00630201845863275", "module": "A1"}, {"value": "2.85710354098807E-05", "module": "A2"}, {"value": "0.000580195147872002", "module": "A3"}, {"value": "4.13898884874543E-05", "module": "A4"}, {"value": "0.000624203780190073", "module": "A5"}, {"value": "1.84998338390185E-05", "module": "C1"}, {"value": "2.79358852928974E-06", "module": "C2"}, {"value": "0", "module": "C3"}, {"value": "0.00213715646120998", "module": "C4"}, {"value": "0", "module": "D"}]}}, {"referenceToLCIAMethodDataSet": {"shortDescription": [{"value": "Eutrophication potential terrestrial (EP-terrestrial)", "lang": "en"}, {"value": "Eutrophierungspotenzial Land (EP-terrestrial)", "lang": "de"}], "type": "LCIA method data set", "refObjectId": "b5c614d2-def3-11e6-bf01-fe55135034f3", "uri": "../lciamethods/b5c614d2-def3-11e6-bf01-fe55135034f3.xml"}, "other": {"anies": [{"name": "referenceToUnitGroupDataSet", "value": {"shortDescription": [{"value": "mol N-Äq.", "lang": "en"}], "type": "unit group data set", "refObjectId": "71b4d617-0ec9-4d3f-b65e-e438940c2401", "uri": "../unitgroups/71b4d617-0ec9-4d3f-b65e-e438940c2401.xml"}}, {"value": "0.0391623630690459", "module": "A1"}, {"value": "0.00031027066388411", "module": "A2"}, {"value": "0.00435955749372099", "module": "A3"}, {"value": "0.000449478571387391", "module": "A4"}, {"value": "0.00624881933399791", "module": "A5"}, {"value": "0.000202619824632486", "module": "C1"}, {"value": "3.0337317327394E-05", "module": "C2"}, {"value": "0", "module": "C3"}, {"value": "0.000306745458873782", "module": "C4"}, {"value": "0", "module": "D"}]}}, {"referenceToLCIAMethodDataSet": {"shortDescription": [{"value": "Formation potential of tropospheric ozone photochemical oxidants (POCP)", "lang": "en"}, {"value": "Bildungspotential für troposphärisches Ozon (POCP)", "lang": "de"}], "type": "LCIA method data set", "refObjectId": "b5c610fe-def3-11e6-bf01-fe55135034f3", "uri": "../lciamethods/b5c610fe-def3-11e6-bf01-fe55135034f3.xml"}, "other": {"anies": [{"name": "referenceToUnitGroupDataSet", "value": {"shortDescription": [{"value": "kg NMVOC-Äq.", "lang": "en"}], "type": "unit group data set", "refObjectId": "d27c25f8-fbc1-44c6-b47b-4adbae4199c6", "uri": "../unitgroups/d27c25f8-fbc1-44c6-b47b-4adbae4199c6.xml"}}, {"value": "0.0144803101193009", "module": "A1"}, {"value": "0.000119209215593051", "module": "A2"}, {"value": "0.00133671682502573", "module": "A3"}, {"value": "0.000172694341289674", "module": "A4"}, {"value": "0.00148324038497632", "module": "A5"}, {"value": "5.57190057263494E-05", "module": "C1"}, {"value": "1.16559127973082E-05", "module": "C2"}, {"value": "0", "module": "C3"}, {"value": "0.0001117727461649", "module": "C4"}, {"value": "0", "module": "D"}]}}, {"referenceToLCIAMethodDataSet": {"shortDescription": [{"value": "Abiotic depletion potential for non fossil resources (ADPE)", "lang": "en"}, {"value": "Potenzial für den abiotischen Abbau nicht fossiler Ressourcen (ADPE)", "lang": "de"}], "type": "LCIA method data set", "refObjectId": "b2ad6494-c78d-11e6-9d9d-cec0c932ce01", "uri": "../lciamethods/b2ad6494-c78d-11e6-9d9d-cec0c932ce01.xml"}, "other": {"anies": [{"name": "referenceToUnitGroupDataSet", "value": {"shortDescription": [{"value": "kg Sb-Äq.", "lang": "en"}], "type": "unit group data set", "refObjectId": "54ccd2d9-a32a-4fc2-923d-f2c8c93e89d4", "uri": "../unitgroups/54ccd2d9-a32a-4fc2-923d-f2c8c93e89d4.xml"}}, {"value": "4.45677777339765E-05", "module": "A1"}, {"value": "1.7809423121809E-07", "module": "A2"}, {"value": "1.7517591298099E-06", "module": "A3"}, {"value": "2.57999063199034E-07", "module": "A4"}, {"value": "7.85070612093543E-06", "module": "A5"}, {"value": "2.03521771763841E-09", "module": "C1"}, {"value": "1.74135096725082E-08", "module": "C2"}, {"value": "0", "module": "C3"}, {"value": "3.11122707227237E-08", "module": "C4"}, {"value": "0", "module": "D"}]}}, {"referenceToLCIAMethodDataSet": {"shortDescription": [{"value": "Abiotic depletion potential for fossil resources (ADPF)", "lang": "en"}, {"value": "Potenzial für den abiotischen Abbau fossiler Brennstoffe (ADPF)", "lang": "de"}], "type": "LCIA method data set", "refObjectId": "b2ad6110-c78d-11e6-9d9d-cec0c932ce01", "uri": "../lciamethods/b2ad6110-c78d-11e6-9d9d-cec0c932ce01.xml"}, "other": {"anies": [{"name": "referenceToUnitGroupDataSet", "value": {"shortDescription": [{"value": "MJ", "lang": "en"}], "type": "unit group data set", "refObjectId": "93a60a57-a3c8-11da-a746-0800200c9a66", "uri": "../unitgroups/93a60a57-a3c8-11da-a746-0800200c9a66.xml"}}, {"value": "58.0225288176827", "module": "A1"}, {"value": "0.733378930253049", "module": "A2"}, {"value": "8.31721004271022", "module": "A3"}, {"value": "1.06242114458774", "module": "A4"}, {"value": "6.46458199048864", "module": "A5"}, {"value": "0.0540548656353868", "module": "C1"}, {"value": "0.071707550594025", "module": "C2"}, {"value": "0", "module": "C3"}, {"value": "0.221985178737816", "module": "C4"}, {"value": "0", "module": "D"}]}}, {"referenceToLCIAMethodDataSet": {"shortDescription": [{"value": "Water use (WDP)", "lang": "en"}, {"value": "Wassernutzung (WDP)", "lang": "de"}], "type": "LCIA method data set", "refObjectId": "b2ad66ce-c78d-11e6-9d9d-cec0c932ce01", "uri": "../lciamethods/b2ad66ce-c78d-11e6-9d9d-cec0c932ce01.xml"}, "other": {"anies": [{"name": "referenceToUnitGroupDataSet", "value": {"shortDescription": [{"value": "m^(3) world-Äq. deprived", "lang": "en"}], "type": "unit group data set", "refObjectId": "6ae2df01-888e-46c8-b17d-49fa3869b476", "uri": "../unitgroups/6ae2df01-888e-46c8-b17d-49fa3869b476.xml"}}, {"value": "5.47098280410804", "module": "A1"}, {"value": "0.00343254807247315", "module": "A2"}, {"value": "0.231819163966357", "module": "A3"}, {"value": "0.00497261579460846", "module": "A4"}, {"value": "0.456158292723535", "module": "A5"}, {"value": "0.000145261403238191", "module": "C1"}, {"value": "0.000335624060659013", "module": "C2"}, {"value": "0", "module": "C3"}, {"value": "0.00230065643481459", "module": "C4"}, {"value": "0", "module": "D"}]}}, {"referenceToLCIAMethodDataSet": {"shortDescription": [{"value": "Incidence of disease due to PM emissions (PM)", "lang": "en"}, {"value": "Auftreten von Krankheiten aufgrund von Feinstaubemissionen (PM)", "lang": "de"}], "type": "LCIA method data set", "refObjectId": "b5c602c6-def3-11e6-bf01-fe55135034f3", "uri": "../lciamethods/b5c602c6-def3-11e6-bf01-fe55135034f3.xml"}, "other": {"anies": [{"name": "referenceToUnitGroupDataSet", "value": {"shortDescription": [{"value": "Disease incidence", "lang": "en"}], "type": "unit group data set", "refObjectId": "3883559b-648f-4afc-8ba2-0bd24f3affa3", "uri": "../unitgroups/3883559b-648f-4afc-8ba2-0bd24f3affa3.xml"}}, {"value": "1.58510405374853E-07", "module": "A1"}, {"value": "3.97101315774574E-09", "module": "A2"}, {"value": "2.34386092221093E-08", "module": "A3"}, {"value": "5.75267187287409E-09", "module": "A4"}, {"value": "2.35166250128893E-08", "module": "A5"}, {"value": "1.11873868478358E-09", "module": "C1"}, {"value": "3.88273531147588E-10", "module": "C2"}, {"value": "0", "module": "C3"}, {"value": "1.62228294532332E-09", "module": "C4"}, {"value": "0", "module": "D"}]}}, {"referenceToLCIAMethodDataSet": {"shortDescription": [{"value": "Human exposure efficiency relative to U235 (IR)", "lang": "en"}, {"value": "Wirkung durch Exposition des Menschen mit U235 (IR)", "lang": "de"}], "type": "LCIA method data set", "refObjectId": "b5c632be-def3-11e6-bf01-fe55135034f3", "uri": "../lciamethods/b5c632be-def3-11e6-bf01-fe55135034f3.xml"}, "other": {"anies": [{"name": "referenceToUnitGroupDataSet", "value": {"shortDescription": [{"value": "kBq U235-Äq.", "lang": "en"}], "type": "unit group data set", "refObjectId": "456b05bf-1415-44a9-9993-02452f554c09", "uri": "../unitgroups/456b05bf-1415-44a9-9993-02452f554c09.xml"}}, {"value": "0.249717445289365", "module": "A1"}, {"value": "0.00384839132238316", "module": "A2"}, {"value": "0.0351434962538287", "module": "A3"}, {"value": "0.00557503378524535", "module": "A4"}, {"value": "0.0322077088301957", "module": "A5"}, {"value": "0.000248375137430415", "module": "C1"}, {"value": "0.000376283942818181", "module": "C2"}, {"value": "0", "module": "C3"}, {"value": "0.00147816480193856", "module": "C4"}, {"value": "0", "module": "D"}]}}, {"referenceToLCIAMethodDataSet": {"shortDescription": [{"value": "Comparative toxic unit for ecosystems (ETP-fw)", "lang": "en"}, {"value": "Toxizitätsvergleichseinheit für Ökosysteme (ETP-fw)", "lang": "de"}], "type": "LCIA method data set", "refObjectId": "ee1082d1-b0f7-43ca-a1f0-21e2a4a74511", "uri": "../lciamethods/ee1082d1-b0f7-43ca-a1f0-21e2a4a74511.xml"}, "other": {"anies": [{"name": "referenceToUnitGroupDataSet", "value": {"shortDescription": [{"value": "CTUe", "lang": "en"}], "type": "unit group data set", "refObjectId": "aa959ded-f1eb-4efb-9c5c-2d60be36b3e6", "uri": "../unitgroups/aa959ded-f1eb-4efb-9c5c-2d60be36b3e6.xml"}}, {"value": "159.871965354273", "module": "A1"}, {"value": "0.6120680600168", "module": "A2"}, {"value": "6.49189286224076", "module": "A3"}, {"value": "0.886682207606198", "module": "A4"}, {"value": "20.2193057630198", "module": "A5"}, {"value": "0.0324899190412773", "module": "C1"}, {"value": "0.0598461444283617", "module": "C2"}, {"value": "0", "module": "C3"}, {"value": "0.482533379471391", "module": "C4"}, {"value": "0", "module": "D"}]}}, {"referenceToLCIAMethodDataSet": {"shortDescription": [{"value": "Comparative toxic unit for humans (carcinogenic) (HTP-c)", "lang": "en"}, {"value": "Toxizitätsvergleichseinheit für Menschen (krebserregend) (HTP-c)", "lang": "de"}], "type": "LCIA method data set", "refObjectId": "2299222a-bbd8-474f-9d4f-4dd1f18aea7c", "uri": "../lciamethods/2299222a-bbd8-474f-9d4f-4dd1f18aea7c.xml"}, "other": {"anies": [{"name": "referenceToUnitGroupDataSet", "value": {"shortDescription": [{"value": "CTUh", "lang": "en"}], "type": "unit group data set", "refObjectId": "d4c9523e-2d7e-49fd-8469-998f547d3a70", "uri": "../unitgroups/d4c9523e-2d7e-49fd-8469-998f547d3a70.xml"}}, {"value": "6.09006027313543E-09", "module": "A1"}, {"value": "1.88144086252008E-11", "module": "A2"}, {"value": "2.30066161479906E-10", "module": "A3"}, {"value": "2.7255794680971E-11", "module": "A4"}, {"value": "6.71457141232433E-10", "module": "A5"}, {"value": "1.2452562026263E-12", "module": "C1"}, {"value": "1.83961537853662E-12", "module": "C2"}, {"value": "0", "module": "C3"}, {"value": "7.11842389144528E-12", "module": "C4"}, {"value": "0", "module": "D"}]}}, {"referenceToLCIAMethodDataSet": {"shortDescription": [{"value": "Comparative toxic unit for humans (noncarcinogenic) (HTP-nc)", "lang": "en"}, {"value": "Toxizitätsvergleichseinheit für Menschen (nicht krebserregend) (HTP-nc)", "lang": "de"}], "type": "LCIA method data set", "refObjectId": "3af763a5-b7a1-48c9-9cee-1f223481fcef", "uri": "../lciamethods/3af763a5-b7a1-48c9-9cee-1f223481fcef.xml"}, "other": {"anies": [{"name": "referenceToUnitGroupDataSet", "value": {"shortDescription": [{"value": "CTUh", "lang": "en"}], "type": "unit group data set", "refObjectId": "d4c9523e-2d7e-49fd-8469-998f547d3a70", "uri": "../unitgroups/d4c9523e-2d7e-49fd-8469-998f547d3a70.xml"}}, {"value": "8.99013266264874E-06", "module": "A1"}, {"value": "5.99139030258615E-10", "module": "A2"}, {"value": "1.09494236806332E-08", "module": "A3"}, {"value": "8.67952361373282E-10", "module": "A4"}, {"value": "6.33160446580382E-07", "module": "A5"}, {"value": "2.3490070794889E-11", "module": "C1"}, {"value": "5.85819834097232E-11", "module": "C2"}, {"value": "0", "module": "C3"}, {"value": "1.80610945869833E-10", "module": "C4"}, {"value": "0", "module": "D"}]}}, {"referenceToLCIAMethodDataSet": {"shortDescription": [{"value": "Soil quality index (SQP)", "lang": "en"}, {"value": "Bodenqualitätsindex (SQP)", "lang": "de"}], "type": "LCIA method data set", "refObjectId": "b2ad6890-c78d-11e6-9d9d-cec0c932ce01", "uri": "../lciamethods/b2ad6890-c78d-11e6-9d9d-cec0c932ce01.xml"}, "other": {"anies": [{"name": "referenceToUnitGroupDataSet", "value": {"shortDescription": [{"value": "SQP", "lang": "en"}], "type": "unit group data set", "refObjectId": "f130951c-e67f-4f7f-8dd4-665de3974e18", "uri": "../unitgroups/f130951c-e67f-4f7f-8dd4-665de3974e18.xml"}}, {"value": "44.8019823841332", "module": "A1"}, {"value": "0.520858110738912", "module": "A2"}, {"value": "4.42537455283417", "module": "A3"}, {"value": "0.754549452338512", "module": "A4"}, {"value": "3.97874493896146", "module": "A5"}, {"value": "0.00702558821175943", "module": "C1"}, {"value": "0.0509279143255882", "module": "C2"}, {"value": "0", "module": "C3"}, {"value": "0.58299302655433", "module": "C4"}, {"value": "0", "module": "D"}]}}]}, "otherAttributes": {"{http://www.indata.network/EPD/2019}epd-version": "1.2"}, "version": "1.1", "locations": "../ILCDLocations.xml"}