{"processInformation": {"dataSetInformation": {"UUID": "22185222-4f46-4180-b940-46f23408057e", "name": {"baseName": [{"value": "Rahmenprofile für Fenster - heroal-Johann Henkenjohann GmbH & Co. KG - Hebeschiebeelement (EN 15804+A2)", "lang": "de"}, {"value": "Frame Profiles for Windows - heroal-Johann Henkenjohann GmbH & Co. KG - lifting-sliding elements (EN 15804+A2)", "lang": "en"}, {"value": "Profilés de châssis pour fenêtres - heroal-Johann Henkenjohann GmbH & Co. KG - Élément coulissant à levage (EN 15804+A2)", "lang": "fr"}, {"value": "Profili per telaio per finestre - heroal-Johann Henkenjohann GmbH & Co. KG - Elemento alzante-scorrevole (EN 15804+A2)", "lang": "it"}]}, "synonyms": [{"value": "Aluminium-Fenstersysteme; Hebeschiebetür; Hebe-Schiebetür; Hebe-Schiebetürsystem; S65; S42; S77; W72 PSK", "lang": "de"}, {"value": "aluminium window systems; lifting-sliding door; lifting door; lifting-sliding door system; S65; S42; S77; W72; PSK", "lang": "en"}, {"value": "systèmes de fenêtre en aluminium; portes coulissantes; S65; S42; S77; W72 PSK", "lang": "fr"}, {"value": "Sistemi per finestre in alluminio; sistema per porte alzanti-scorrevoli; S65; S42; S77; W72 PSK", "lang": "it"}], "classificationInformation": {"classification": [{"class": [{"value": "Komponenten von Fenstern und Vorhangfassaden", "level": 0, "classId": "7"}, {"value": "Rahmen / Profile", "level": 1, "classId": "7.1"}, {"value": "Aluminium thermisch getrennt", "level": 2, "classId": "7.1.06"}], "name": "OEKOBAU.DAT"}]}, "generalComment": [{"value": "Aluminiumprofile mit Bautiefen bon 77 mm bis 202 mm.\r\nAnsichtsbreiten von 35 mm bis 52 mm.\r\n\r\nA1-A3 sowie Module A4, A5, B2, B3, B4, B5, B6, B7, C1, C2, C3, C4, D. Das Umweltprofil beinhaltet die Aufwendungen für die Lebenszyklus-Stadien cradle to gate mit Optionen (Modul A1-A3). Die Herstellung der Verpackung wurde innerhalb der Module A1-A3 berücksichtigt.", "lang": "de"}, {"value": "aluminium profiles with installation depths from 77 mm to 202 mm. Face widths from 35 mm to 52 mm.\r\n\r\nA1-A3 as well as modules A4, A5, B2, B3, B4, B5, B6, B7, C1, C2, C3, C4, D. The environmental profile includes the expenditures for the life cycle stages cradle to gate with options (module A1-A3). The production of the packaging was taken into account within modules A1-A3.", "lang": "en"}]}, "quantitativeReference": {"referenceToReferenceFlow": [1], "type": "Reference flow(s)"}, "time": {"referenceYear": 2021, "dataSetValidUntil": 2026, "timeRepresentativenessDescription": [{"value": "jährlicher Durchschnitt", "lang": "de"}, {"value": "anual average", "lang": "en"}], "other": {"anies": [{"name": "publicationDateOfEPD", "value": 1618444800000}]}}, "geography": {"locationOfOperationSupplyOrProduction": {"descriptionOfRestrictions": [{"value": "Dieser Datensatz repräsentiert die Situation des Unternehmens heroal-Johann Henkenjohann GmbH & Co. KG in 33415 Verl im Hinblick auf die wichtigsten Technologien und die gesetzlichen Rahmenbedingungen.", "lang": "de"}, {"value": "This data set represents the situation of heroal-Johann Henkenjohann GmbH & Co. KG in 33415 Verl, with regard to the most important technologies and the legal framework.", "lang": "en"}], "location": "DE"}}, "technology": {"technologyDescriptionAndIncludedProcesses": [{"value": "Die Ökobilanzergebnisse umfassen die Lebenszyklusstadien der Herstellung der Vorprodukte bis hin zur Rohstoffgewinnung und Verarbeitungsprozesse von als Input dienenden Sekundärstoffen (z.B. Recyclingprozesse), deren Transporte zum Werk sowie die Produktion selbst, einschließlich der Bereitstellung von allen Hilfs- und Betriebsstoffen, Energie, sowie die vollständige Abfallbehandlung oder die Deponierung der Restabfälle während des Stadiums der Produktion. Die Module A1, A2 und A3 sind hier als ein aggregiertes Modul A1-A3 ausgewiesen. Falls für diesen Datensatz weitere Module berechnet wurden, sind diese separat zu finden und können für eine Betrachtung des gesamten Lebenszyklus zusammengeführt werden.", "lang": "de"}, {"value": "The LCA results include the life cycle stages of the pre-products manufacture to the point of the raw material extraction and processing of secondary material input (e.g. recycling processes), their transport to the manufacturer as well as the maufacturing itself, including provision of all operating supplies, energy and the complete waste treatment or the landfill of residual waste during the stage of manufacture.\r\nThe modules A1, A2 and A3 are shown here as an aggregated module A1-A3. If further modules have been calculated for this dataset, these can be found separately and can be merged for consideration of the entire life cycle.", "lang": "en"}], "technologicalApplicability": [{"value": "Hebe-Schiebetürsysteme aus Aluminium für alle Gebäudeklassen.", "lang": "de"}, {"value": "Aluminium lifting-sliding door systems for all building classes ", "lang": "en"}, {"value": "Systèmes de portes coulissantes à levage  en aluminium pour toutes les classes de bâtiment.", "lang": "fr"}, {"value": "Sistemi per porte alzanti-scorrevoli in alluminio per tutte le classi di edifici.", "lang": "it"}]}}, "modellingAndValidation": {"LCIMethodAndAllocation": {"typeOfDataSet": "EPD", "referenceToLCAMethodDetails": [{"shortDescription": [{"value": "Produktkategorieregeln Teil A", "lang": "de"}], "type": "source data set", "refObjectId": "c6e986be-62a9-4f2f-b486-27aa9129eaeb", "version": "00.00.006"}, {"shortDescription": [{"value": "Produktkategorieregeln Teil B – für Profile für Fenster, Türen und Fassaden", "lang": "de"}], "type": "source data set", "refObjectId": "378990bd-bd0e-4d79-b450-f933a2c6d0f8", "version": "00.00.004"}], "other": {"anies": [{"name": "subType", "value": "specific dataset"}]}}, "dataSourcesTreatmentAndRepresentativeness": {"referenceToDataSource": [{"shortDescription": [{"value": "GaBi database (general)", "lang": "en"}], "type": "source data set", "refObjectId": "28d74cc0-db8b-4d7e-bc44-5f6d56ce0c4a", "version": "00.03.003"}], "useAdviceForDataSet": [{"value": "Dieser Datensatz beinhaltet die Ergebnisse für die Module A1-A3 sowie die Module A4, A5, B2, B3, B4, B5, B6, B7, C1, C2, C3, C4, D gemäß EN 15804.\r\nEin Vergleich mit anderen Produkten ist nur mit einer vergleichbaren Anwendung im Gebäude zulässig. Grundsätzlich ist eine Gegenüberstellung oder die Bewertung von EPD Daten nur möglich, wenn alle zu vergleichenden Datensätze nach EN 15804 erstellt wurden und der Gebäudekontext, bzw. die produktspezifischen Leistungsmerkmale berücksichtigt werden.", "lang": "de"}, {"value": "The comparison with other products is only permissible if the application in the building is comparable. A comparison or the evaluation of EPD data is only possible, if the datasets have been created according to EN 15804. The building context or the product-specific performance characteristics must be considered.", "lang": "en"}], "other": {"anies": [{"name": "referenceToOriginalEPD", "value": {"shortDescription": {"value": "EPD Rahmenprofile für Aluminiumfenster und -türen  - heroal-Johann Henkenjohann GmbH & Co. KG", "defaultValue": "EPD Rahmenprofile für Aluminiumfenster und -türen  - heroal-Johann Henkenjohann GmbH & Co. KG", "lstrings": [{"lang": "de", "value": "EPD Rahmenprofile für Aluminiumfenster und -türen  - heroal-Johann Henkenjohann GmbH & Co. KG"}]}, "version": {"version": 1, "majorVersion": 0, "minorVersion": 0, "subMinorVersion": 1, "zero": false, "versionString": "00.00.001"}, "type": "source data set", "uuid": {"uuid": "8f021a73-6cb4-470c-b090-0e5d00b2c871"}, "refObjectId": "8f021a73-6cb4-470c-b090-0e5d00b2c871", "versionAsString": "00.00.001", "resourceURLs": ["https://oekobaudat.de/OEKOBAU.DAT/resource/sources/8f021a73-6cb4-470c-b090-0e5d00b2c871/EPD-AFT-IT-38.0.pdf?version=00.00.001", "https://oekobaudat.de/OEKOBAU.DAT/resource/sources/8f021a73-6cb4-470c-b090-0e5d00b2c871/EPD-AFT-38.0.pdf?version=00.00.001", "https://oekobaudat.de/OEKOBAU.DAT/resource/sources/8f021a73-6cb4-470c-b090-0e5d00b2c871/EPD-AFT-FR-38.0.pdf?version=00.00.001", "https://oekobaudat.de/OEKOBAU.DAT/resource/sources/8f021a73-6cb4-470c-b090-0e5d00b2c871/EPD-AFT-GB-38.0.pdf?version=00.00.001"]}}]}}, "validation": {"review": [{"reviewDetails": [{"value": "Die angewendete LCI Methode ist in Übereinstimmung mit ISO 14040 und 14044. Die Dokumentation enthält alle relevanten Informationen im Hinblick auf die Datenqualität und den Umfang der Anwendung der jeweiligen LCI Ergebnisse bzw. der Datensätze. Der Datensatz repräsentiert den Stand der Technik bezogen auf die funktionelle Einheit.", "lang": "de"}, {"value": "The LCI method applied is in compliance with ISO 14040 and 14044. The documentation includes all relevant information in view of the data quality and scope of the application of the respective LCI result / data set. The dataset represents the state-of-the-art in view of the referenced functional unit.", "lang": "en"}], "referenceToNameOfReviewerAndInstitution": [{"shortDescription": [{"value": "Patrick Wortner", "lang": "de"}, {"value": "Patrick Wortner", "lang": "en"}], "type": "contact data set", "refObjectId": "4ca8370d-bd95-4619-9fe3-8c74f628b623", "version": "00.00.003", "uri": "http://openlca.org/ilcd/resource/contacts/4ca8370d-bd95-4619-9fe3-8c74f628b623"}], "type": "Independent external review"}]}, "complianceDeclarations": {"compliance": [{"referenceToComplianceSystem": {"shortDescription": [{"value": "EN 15804+A2", "lang": "de"}, {"value": "EN 15804+A2", "lang": "en"}], "type": "source data set", "refObjectId": "c0016b33-8cf7-415c-ac6e-deba0d21440d", "version": "00.01.002"}}]}}, "administrativeInformation": {"dataGenerator": {"referenceToPersonOrEntityGeneratingTheDataSet": [{"shortDescription": [{"value": "ift Rosenheim", "lang": "en"}], "type": "contact data set", "refObjectId": "e4e77c13-c6e7-437a-8b76-826e43bb5a95", "version": "00.00.001", "uri": "http://openlca.org/ilcd/resource/contacts/e4e77c13-c6e7-437a-8b76-826e43bb5a95"}]}, "dataEntryBy": {"timeStamp": 1734364359210, "referenceToDataSetFormat": [{"shortDescription": [{"value": "ILCD format", "lang": "en"}], "type": "source data set", "refObjectId": "a97a0155-0234-4b87-b4ce-a45da52f2a40", "version": "03.01.004", "uri": "http://lca.jrc.ec.europa.eu/lcainfohub/datasets/ilcd/sources/a97a0155-0234-4b87-b4ce-a45da52f2a40.xml"}, {"shortDescription": [{"value": "EPD Data Format Extensions v1.2", "lang": "en"}, {"value": "EPD-Datenformaterweiterungen v1.2", "lang": "de"}], "type": "source data set", "refObjectId": "a29449fd-aa2f-4de8-b5d7-4b06b43c6fde", "version": "00.01.003"}], "referenceToPersonOrEntityEnteringTheData": {"shortDescription": [{"value": "ift Rosenheim", "lang": "en"}], "type": "contact data set", "refObjectId": "e4e77c13-c6e7-437a-8b76-826e43bb5a95", "version": "00.00.001", "uri": "http://openlca.org/ilcd/resource/contacts/e4e77c13-c6e7-437a-8b76-826e43bb5a95"}}, "publicationAndOwnership": {"dataSetVersion": "00.00.049", "referenceToRegistrationAuthority": {"shortDescription": [{"value": "ift Rosenheim", "lang": "en"}], "type": "contact data set", "refObjectId": "e4e77c13-c6e7-437a-8b76-826e43bb5a95", "version": "00.00.001", "uri": "http://openlca.org/ilcd/resource/contacts/e4e77c13-c6e7-437a-8b76-826e43bb5a95"}, "registrationNumber": "EPD-AFT-38.0", "referenceToOwnershipOfDataSet": {"shortDescription": [{"value": "heroal-Johann Henkenjohann GmbH Co. KG", "lang": "de"}, {"value": "heroal-Johann Henkenjohann GmbH Co. KG", "lang": "en"}], "type": "contact data set", "refObjectId": "ede7e0ab-d256-4e23-96d4-3fd10219d5c0", "version": "00.01.007"}, "copyright": true, "licenseType": "Free of charge for all users and uses", "accessRestrictions": [{"value": "None.", "lang": "de"}], "other": {"anies": [{"name": "referenceToPublisher", "value": {"shortDescription": [{"value": "The Federal Institute for Research on Building, Urban Affairs and Spatial Development (BBSR) within the Federal Office for Building and Regional Planning (BBR)", "lang": "en"}, {"value": "Bundesinstitut für Bau-, Stadt- und Raumforschung (BBSR) im Bundesamt für Bauwesen und Raumordnung (BBR) ", "lang": "de"}], "type": "contact data set", "refObjectId": "f11651e0-7877-11e3-981f-0800200c9a66", "version": "00.01.000"}}]}}}, "exchanges": {"exchange": [{"dataSetInternalID": 1, "referenceToFlowDataSet": {"shortDescription": [{"value": "Rahmenprofile für Fenster - heroal-Johann Henkenjohann GmbH & Co. KG - Hebeschiebeelement (EN 15804+A2)", "lang": "de"}, {"value": "Frame Profiles for Windows - heroal-Johann Henkenjohann GmbH & Co. KG - lifting-sliding elements (EN 15804+A2)", "lang": "en"}, {"value": "Profilés de châssis pour fenêtres - heroal-Johann Henkenjohann GmbH & Co. KG - Élément coulissant à levage (EN 15804+A2)", "lang": "fr"}, {"value": "Profili per telaio per finestre - heroal-Johann Henkenjohann GmbH & Co. KG - Elemento alzante-scorrevole (EN 15804+A2)", "lang": "it"}], "type": "flow data set", "refObjectId": "038b4530-56b8-4810-a011-44f95fd8c276", "version": "00.00.020"}, "meanAmount": 1.0, "resultingAmount": 1.0, "referenceFlow": true, "resultingflowAmount": 1.0, "flowProperties": [{"name": [{"lang": "de", "value": "Biogener Kohlenstoffgehalt in der zugehörigen Verpackung (Biog. C in packaging)"}, {"lang": "en", "value": "Biogenic carbon content in accompanying packaging (Biog. C in packaging)"}], "uuid": "262a541b-209e-44cc-a426-33bce30de7b1", "meanValue": 0.03}, {"name": [{"lang": "de", "value": "Länge"}, {"lang": "en", "value": "Length"}], "uuid": "838aaa23-0117-11db-92e3-0800200c9a66", "referenceFlowProperty": true, "meanValue": 1.0, "referenceUnit": "m", "unitGroupUUID": "838aaa22-0117-11db-92e3-0800200c9a66"}], "materialProperties": [{"name": "linear density", "value": "2.9", "unit": "kg/m"}], "typeOfFlow": "Product flow", "classification": {"classHierarchy": "Komponenten von Fenstern und Vorhangfassaden / Rahmen / Profile / Aluminium thermisch getrennt", "name": "OEKOBAU.DAT"}}, {"dataSetInternalID": 2, "referenceToFlowDataSet": {"shortDescription": [{"value": "Components for re-use (CRU)", "lang": "en"}, {"value": "Komponenten für die Wiederverwendung (CRU)", "lang": "de"}], "type": "flow data set", "refObjectId": "a2b32f97-3fc7-4af2-b209-525bc6426f33", "version": "38.00.000"}, "exchange direction": "OUTPUT", "meanAmount": 0.0, "other": {"anies": [{"value": "0.0", "module": "A1-A3"}, {"value": "0.0", "module": "A4"}, {"value": "0.0", "module": "A5"}, {"module": "B1"}, {"value": "0.0", "module": "B2"}, {"value": "0.0", "module": "B3"}, {"value": "0.0", "module": "B4"}, {"value": "0.0", "module": "B5"}, {"value": "0.0", "module": "B6"}, {"value": "0.0", "module": "B7"}, {"value": "0.0", "module": "C1"}, {"value": "0.0", "module": "C2"}, {"value": "0.0", "module": "C3"}, {"value": "0.0", "module": "C4"}, {"value": "0.0", "module": "D"}, {"name": "referenceToUnitGroupDataSet", "value": {"shortDescription": [{"value": "kg"}], "type": "unit group data set", "refObjectId": "ad38d542-3fe9-439d-9b95-2f5f7752acaf", "uri": "../unitgroups/ad38d542-3fe9-439d-9b95-2f5f7752acaf"}}]}, "flowProperties": [], "typeOfFlow": "Other flow", "classification": {"classHierarchy": "Quantities / Environmental quantities / EPD EN 15804 / LCI indicators", "name": "GaBiCategories"}}, {"dataSetInternalID": 3, "referenceToFlowDataSet": {"shortDescription": [{"value": "Exported electrical energy (EEE)", "lang": "en"}, {"value": "Exportierte elektrische Energie (EEE)", "lang": "de"}], "type": "flow data set", "refObjectId": "4da0c987-2b76-40d6-9e9e-82a017aaaf29", "version": "38.00.000"}, "exchange direction": "OUTPUT", "meanAmount": 0.0, "other": {"anies": [{"value": "0.15", "module": "A1-A3"}, {"value": "0.0", "module": "A4"}, {"value": "0.25", "module": "A5"}, {"module": "B1"}, {"value": "1.63", "module": "B2"}, {"value": "0.0", "module": "B3"}, {"value": "0.0", "module": "B4"}, {"value": "4.48", "module": "B5"}, {"value": "0.0", "module": "B6"}, {"value": "0.0", "module": "B7"}, {"value": "0.0", "module": "C1"}, {"value": "0.0", "module": "C2"}, {"value": "4.08", "module": "C3"}, {"value": "0.0", "module": "C4"}, {"value": "0.0", "module": "D"}, {"name": "referenceToUnitGroupDataSet", "value": {"shortDescription": [{"value": "MJ"}], "type": "unit group data set", "refObjectId": "93a60a57-a3c8-11da-a746-0800200c9a66", "uri": "../unitgroups/93a60a57-a3c8-11da-a746-0800200c9a66"}}]}, "flowProperties": [], "typeOfFlow": "Other flow", "classification": {"classHierarchy": "Quantities / Environmental quantities / EPD EN 15804 / LCI indicators", "name": "GaBiCategories"}}, {"dataSetInternalID": 4, "referenceToFlowDataSet": {"shortDescription": [{"value": "Exported thermal energy (EET)", "lang": "en"}, {"value": "Exportierte thermische Energie (EET)", "lang": "de"}], "type": "flow data set", "refObjectId": "98daf38a-7a79-46d3-9a37-2b7bd0955810", "version": "38.00.000"}, "exchange direction": "OUTPUT", "meanAmount": 0.0, "other": {"anies": [{"value": "0.34", "module": "A1-A3"}, {"value": "0.0", "module": "A4"}, {"value": "0.44", "module": "A5"}, {"module": "B1"}, {"value": "2.9", "module": "B2"}, {"value": "0.0", "module": "B3"}, {"value": "0.0", "module": "B4"}, {"value": "8.04", "module": "B5"}, {"value": "0.0", "module": "B6"}, {"value": "0.0", "module": "B7"}, {"value": "0.0", "module": "C1"}, {"value": "0.0", "module": "C2"}, {"value": "7.26", "module": "C3"}, {"value": "0.0", "module": "C4"}, {"value": "0.0", "module": "D"}, {"name": "referenceToUnitGroupDataSet", "value": {"shortDescription": [{"value": "MJ"}], "type": "unit group data set", "refObjectId": "93a60a57-a3c8-11da-a746-0800200c9a66", "uri": "../unitgroups/93a60a57-a3c8-11da-a746-0800200c9a66"}}]}, "flowProperties": [], "typeOfFlow": "Other flow", "classification": {"classHierarchy": "Quantities / Environmental quantities / EPD EN 15804 / LCI indicators", "name": "GaBiCategories"}}, {"dataSetInternalID": 5, "referenceToFlowDataSet": {"shortDescription": [{"value": "Hazardous waste disposed (HWD)", "lang": "en"}, {"value": "Gefährlicher Abfall zur Beseitigung (HWD)", "lang": "de"}], "type": "flow data set", "refObjectId": "430f9e0f-59b2-46a0-8e0d-55e0e84948fc", "version": "38.00.000"}, "exchange direction": "OUTPUT", "meanAmount": 0.0, "other": {"anies": [{"value": "2.65E-6", "module": "A1-A3"}, {"value": "2.85E-10", "module": "A4"}, {"value": "1.42E-11", "module": "A5"}, {"module": "B1"}, {"value": "9.75E-9", "module": "B2"}, {"value": "0.0", "module": "B3"}, {"value": "0.0", "module": "B4"}, {"value": "2.63E-6", "module": "B5"}, {"value": "0.0", "module": "B6"}, {"value": "0.0", "module": "B7"}, {"value": "0.0", "module": "C1"}, {"value": "7.93E-11", "module": "C2"}, {"value": "3.96E-9", "module": "C3"}, {"value": "7.84E-12", "module": "C4"}, {"value": "-2.35E-8", "module": "D"}, {"name": "referenceToUnitGroupDataSet", "value": {"shortDescription": [{"value": "kg"}], "type": "unit group data set", "refObjectId": "ad38d542-3fe9-439d-9b95-2f5f7752acaf", "uri": "../unitgroups/ad38d542-3fe9-439d-9b95-2f5f7752acaf"}}]}, "flowProperties": [], "typeOfFlow": "Other flow", "classification": {"classHierarchy": "Quantities / Environmental quantities / EPD EN 15804 / LCI indicators", "name": "GaBiCategories"}}, {"dataSetInternalID": 6, "referenceToFlowDataSet": {"shortDescription": [{"value": "Material for Energy Recovery (MER)", "lang": "en"}, {"value": "Stoff für die Energierückgewinnung (MER)", "lang": "de"}], "type": "flow data set", "refObjectId": "59a9181c-3aaf-46ee-8b13-2b3723b6e447", "version": "38.00.000"}, "exchange direction": "OUTPUT", "meanAmount": 0.0, "other": {"anies": [{"value": "0.0", "module": "A1-A3"}, {"value": "0.0", "module": "A4"}, {"value": "0.0", "module": "A5"}, {"module": "B1"}, {"value": "0.0", "module": "B2"}, {"value": "0.0", "module": "B3"}, {"value": "0.0", "module": "B4"}, {"value": "0.0", "module": "B5"}, {"value": "0.0", "module": "B6"}, {"value": "0.0", "module": "B7"}, {"value": "0.0", "module": "C1"}, {"value": "0.0", "module": "C2"}, {"value": "0.0", "module": "C3"}, {"value": "0.0", "module": "C4"}, {"value": "0.0", "module": "D"}, {"name": "referenceToUnitGroupDataSet", "value": {"shortDescription": [{"value": "kg"}], "type": "unit group data set", "refObjectId": "ad38d542-3fe9-439d-9b95-2f5f7752acaf", "uri": "../unitgroups/ad38d542-3fe9-439d-9b95-2f5f7752acaf"}}]}, "flowProperties": [], "typeOfFlow": "Other flow", "classification": {"classHierarchy": "Quantities / Environmental quantities / EPD EN 15804 / LCI indicators", "name": "GaBiCategories"}}, {"dataSetInternalID": 7, "referenceToFlowDataSet": {"shortDescription": [{"value": "Materials for Recycling (MFR)", "lang": "en"}, {"value": "Stoffe zum Recycling (MFR)", "lang": "de"}], "type": "flow data set", "refObjectId": "d7fe48a5-4103-49c8-9aae-b0b5dfdbd6ae", "version": "38.00.000"}, "exchange direction": "OUTPUT", "meanAmount": 0.0, "other": {"anies": [{"value": "0.0356", "module": "A1-A3"}, {"value": "0.0", "module": "A4"}, {"value": "0.0", "module": "A5"}, {"module": "B1"}, {"value": "0.0", "module": "B2"}, {"value": "0.0", "module": "B3"}, {"value": "0.0", "module": "B4"}, {"value": "2.18", "module": "B5"}, {"value": "0.0", "module": "B6"}, {"value": "0.0", "module": "B7"}, {"value": "0.0", "module": "C1"}, {"value": "0.0", "module": "C2"}, {"value": "2.14", "module": "C3"}, {"value": "0.0", "module": "C4"}, {"value": "0.0", "module": "D"}, {"name": "referenceToUnitGroupDataSet", "value": {"shortDescription": [{"value": "kg"}], "type": "unit group data set", "refObjectId": "ad38d542-3fe9-439d-9b95-2f5f7752acaf", "uri": "../unitgroups/ad38d542-3fe9-439d-9b95-2f5f7752acaf"}}]}, "flowProperties": [], "typeOfFlow": "Other flow", "classification": {"classHierarchy": "Quantities / Environmental quantities / EPD EN 15804 / LCI indicators", "name": "GaBiCategories"}}, {"dataSetInternalID": 8, "referenceToFlowDataSet": {"shortDescription": [{"value": "Use of net fresh water (FW)", "lang": "en"}, {"value": "Frischwasserverbrauch (FW)", "lang": "de"}], "type": "flow data set", "refObjectId": "3cf952c8-f3a4-461d-8c96-96456ca62246", "version": "38.00.000"}, "exchange direction": "INPUT", "meanAmount": 0.0, "other": {"anies": [{"value": "0.24", "module": "A1-A3"}, {"value": "8.37E-4", "module": "A4"}, {"value": "3.34E-4", "module": "A5"}, {"module": "B1"}, {"value": "0.012", "module": "B2"}, {"value": "0.0", "module": "B3"}, {"value": "0.0", "module": "B4"}, {"value": "0.15", "module": "B5"}, {"value": "0.0", "module": "B6"}, {"value": "0.0", "module": "B7"}, {"value": "0.0", "module": "C1"}, {"value": "2.33E-4", "module": "C2"}, {"value": "0.00601", "module": "C3"}, {"value": "8.35E-6", "module": "C4"}, {"value": "-0.1", "module": "D"}, {"name": "referenceToUnitGroupDataSet", "value": {"shortDescription": [{"value": "m3"}], "type": "unit group data set", "refObjectId": "cd950537-0a98-4044-9ba7-9f9a68d0a504", "uri": "../unitgroups/cd950537-0a98-4044-9ba7-9f9a68d0a504"}}]}, "flowProperties": [], "typeOfFlow": "Other flow", "classification": {"classHierarchy": "Quantities / Environmental quantities / EPD EN 15804 / LCI indicators", "name": "GaBiCategories"}}, {"dataSetInternalID": 9, "referenceToFlowDataSet": {"shortDescription": [{"value": "Non-hazardous waste disposed (NHWD)", "lang": "en"}, {"value": "Ungefährlicher Abfall zur Beseitigung (NHWD)", "lang": "de"}], "type": "flow data set", "refObjectId": "b29ef66b-e286-4afa-949f-62f1a7b4d7fa", "version": "38.00.000"}, "exchange direction": "OUTPUT", "meanAmount": 0.0, "other": {"anies": [{"value": "5.84", "module": "A1-A3"}, {"value": "0.00138", "module": "A4"}, {"value": "0.00168", "module": "A5"}, {"module": "B1"}, {"value": "0.0223", "module": "B2"}, {"value": "0.0", "module": "B3"}, {"value": "0.0", "module": "B4"}, {"value": "3.06", "module": "B5"}, {"value": "0.0", "module": "B6"}, {"value": "0.0", "module": "B7"}, {"value": "0.0", "module": "C1"}, {"value": "3.82E-4", "module": "C2"}, {"value": "0.0105", "module": "C3"}, {"value": "0.16", "module": "C4"}, {"value": "-2.96", "module": "D"}, {"name": "referenceToUnitGroupDataSet", "value": {"shortDescription": [{"value": "kg"}], "type": "unit group data set", "refObjectId": "ad38d542-3fe9-439d-9b95-2f5f7752acaf", "uri": "../unitgroups/ad38d542-3fe9-439d-9b95-2f5f7752acaf"}}]}, "flowProperties": [], "typeOfFlow": "Other flow", "classification": {"classHierarchy": "Quantities / Environmental quantities / EPD EN 15804 / LCI indicators", "name": "GaBiCategories"}}, {"dataSetInternalID": 10, "referenceToFlowDataSet": {"shortDescription": [{"value": "Nicht-erneuerbare Primärenergie als Energieträger (PENRE)", "lang": "en"}, {"value": "Nicht-erneuerbare Primärenergie als Energieträger (PENRE)", "lang": "de"}], "type": "flow data set", "refObjectId": "ac857178-2b45-46ec-892a-a9a4332f0372", "version": "38.00.000"}, "exchange direction": "INPUT", "meanAmount": 0.0, "other": {"anies": [{"value": "339.62", "module": "A1-A3"}, {"value": "8.02", "module": "A4"}, {"value": "1.3", "module": "A5"}, {"module": "B1"}, {"value": "55.2", "module": "B2"}, {"value": "0.0", "module": "B3"}, {"value": "0.0", "module": "B4"}, {"value": "283.63", "module": "B5"}, {"value": "0.0", "module": "B6"}, {"value": "0.0", "module": "B7"}, {"value": "0.0", "module": "C1"}, {"value": "2.23", "module": "C2"}, {"value": "15.17", "module": "C3"}, {"value": "0.69", "module": "C4"}, {"value": "-89.44", "module": "D"}, {"name": "referenceToUnitGroupDataSet", "value": {"shortDescription": [{"value": "MJ"}], "type": "unit group data set", "refObjectId": "93a60a57-a3c8-11da-a746-0800200c9a66", "uri": "../unitgroups/93a60a57-a3c8-11da-a746-0800200c9a66"}}]}, "flowProperties": [], "typeOfFlow": "Other flow", "classification": {"classHierarchy": "Quantities", "name": "GaBiCategories"}}, {"dataSetInternalID": 11, "referenceToFlowDataSet": {"shortDescription": [{"value": "Nicht-erneuerbare Primärenergie zur stofflichen Nutzung (PENRM)", "lang": "en"}, {"value": "Nicht-erneuerbare Primärenergie zur stofflichen Nutzung (PENRM)", "lang": "de"}], "type": "flow data set", "refObjectId": "1421caa0-679d-4bf4-b282-0eb850ccae27", "version": "38.00.000"}, "exchange direction": "INPUT", "meanAmount": 0.0, "other": {"anies": [{"value": "14.49", "module": "A1-A3"}, {"value": "0.0", "module": "A4"}, {"value": "-1.28", "module": "A5"}, {"module": "B1"}, {"value": "0.0", "module": "B2"}, {"value": "0.0", "module": "B3"}, {"value": "0.0", "module": "B4"}, {"value": "-1.78E-15", "module": "B5"}, {"value": "0.0", "module": "B6"}, {"value": "0.0", "module": "B7"}, {"value": "0.0", "module": "C1"}, {"value": "0.0", "module": "C2"}, {"value": "-12.55", "module": "C3"}, {"value": "-0.66", "module": "C4"}, {"value": "0.0", "module": "D"}, {"name": "referenceToUnitGroupDataSet", "value": {"shortDescription": [{"value": "MJ"}], "type": "unit group data set", "refObjectId": "93a60a57-a3c8-11da-a746-0800200c9a66", "uri": "../unitgroups/93a60a57-a3c8-11da-a746-0800200c9a66"}}]}, "flowProperties": [], "typeOfFlow": "Other flow", "classification": {"classHierarchy": "Quantities", "name": "GaBiCategories"}}, {"dataSetInternalID": 12, "referenceToFlowDataSet": {"shortDescription": [{"value": "Use of non renewable secondary fuels (NRSF)", "lang": "en"}, {"value": "Verbrauch nicht erneuerbarer Sekundärbrennstoffe (NRSF)", "lang": "de"}], "type": "flow data set", "refObjectId": "89def144-d39a-4287-b86f-efde453ddcb2", "version": "38.00.000"}, "exchange direction": "INPUT", "meanAmount": 0.0, "other": {"anies": [{"value": "0.0", "module": "A1-A3"}, {"value": "0.0", "module": "A4"}, {"value": "0.0", "module": "A5"}, {"module": "B1"}, {"value": "0.0", "module": "B2"}, {"value": "0.0", "module": "B3"}, {"value": "0.0", "module": "B4"}, {"value": "0.0", "module": "B5"}, {"value": "0.0", "module": "B6"}, {"value": "0.0", "module": "B7"}, {"value": "0.0", "module": "C1"}, {"value": "0.0", "module": "C2"}, {"value": "0.0", "module": "C3"}, {"value": "0.0", "module": "C4"}, {"value": "0.0", "module": "D"}, {"name": "referenceToUnitGroupDataSet", "value": {"shortDescription": [{"value": "MJ"}], "type": "unit group data set", "refObjectId": "93a60a57-a3c8-11da-a746-0800200c9a66", "uri": "../unitgroups/93a60a57-a3c8-11da-a746-0800200c9a66"}}]}, "flowProperties": [], "typeOfFlow": "Other flow", "classification": {"classHierarchy": "Quantities / Environmental quantities / EPD EN 15804 / LCI indicators", "name": "GaBiCategories"}}, {"dataSetInternalID": 13, "referenceToFlowDataSet": {"shortDescription": [{"value": "Radioactive waste disposed (RWD)", "lang": "en"}, {"value": "Entsorgter radioaktiver Abfall (RWD)", "lang": "de"}], "type": "flow data set", "refObjectId": "3449546e-52ad-4b39-b809-9fb77cea8ff6", "version": "38.00.000"}, "exchange direction": "OUTPUT", "meanAmount": 0.0, "other": {"anies": [{"value": "0.0163", "module": "A1-A3"}, {"value": "1.14E-5", "module": "A4"}, {"value": "1.3E-6", "module": "A5"}, {"module": "B1"}, {"value": "4.0E-4", "module": "B2"}, {"value": "0.0", "module": "B3"}, {"value": "0.0", "module": "B4"}, {"value": "0.0119", "module": "B5"}, {"value": "0.0", "module": "B6"}, {"value": "0.0", "module": "B7"}, {"value": "0.0", "module": "C1"}, {"value": "3.17E-6", "module": "C2"}, {"value": "4.36E-4", "module": "C3"}, {"value": "3.31E-7", "module": "C4"}, {"value": "-0.0053", "module": "D"}, {"name": "referenceToUnitGroupDataSet", "value": {"shortDescription": [{"value": "kg"}], "type": "unit group data set", "refObjectId": "ad38d542-3fe9-439d-9b95-2f5f7752acaf", "uri": "../unitgroups/ad38d542-3fe9-439d-9b95-2f5f7752acaf"}}]}, "flowProperties": [], "typeOfFlow": "Other flow", "classification": {"classHierarchy": "Quantities / Environmental quantities / EPD EN 15804 / LCI indicators", "name": "GaBiCategories"}}, {"dataSetInternalID": 14, "referenceToFlowDataSet": {"shortDescription": [{"value": "Erneuerbare Primärenergie als Energieträger (PERE)", "lang": "en"}, {"value": "Erneuerbare Primärenergie als Energieträger (PERE)", "lang": "de"}], "type": "flow data set", "refObjectId": "20f32be5-0398-4288-9b6d-accddd195317", "version": "38.00.000"}, "exchange direction": "INPUT", "meanAmount": 0.0, "other": {"anies": [{"value": "163.09", "module": "A1-A3"}, {"value": "0.68", "module": "A4"}, {"value": "0.93", "module": "A5"}, {"module": "B1"}, {"value": "3.46", "module": "B2"}, {"value": "0.0", "module": "B3"}, {"value": "0.0", "module": "B4"}, {"value": "122.29", "module": "B5"}, {"value": "0.0", "module": "B6"}, {"value": "0.0", "module": "B7"}, {"value": "0.0", "module": "C1"}, {"value": "0.19", "module": "C2"}, {"value": "1.8", "module": "C3"}, {"value": "0.005", "module": "C4"}, {"value": "-46.46", "module": "D"}, {"name": "referenceToUnitGroupDataSet", "value": {"shortDescription": [{"value": "MJ"}], "type": "unit group data set", "refObjectId": "93a60a57-a3c8-11da-a746-0800200c9a66", "uri": "../unitgroups/93a60a57-a3c8-11da-a746-0800200c9a66"}}]}, "flowProperties": [], "typeOfFlow": "Other flow", "classification": {"classHierarchy": "Quantities", "name": "GaBiCategories"}}, {"dataSetInternalID": 15, "referenceToFlowDataSet": {"shortDescription": [{"value": "Erneuerbare Primärenergie zur stofflichen Nutzung (PERM)", "lang": "en"}, {"value": "Erneuerbare Primärenergie zur stofflichen Nutzung (PERM)", "lang": "de"}], "type": "flow data set", "refObjectId": "fb3ec0de-548d-4508-aea5-00b73bf6f702", "version": "38.00.000"}, "exchange direction": "INPUT", "meanAmount": 0.0, "other": {"anies": [{"value": "0.92", "module": "A1-A3"}, {"value": "0.0", "module": "A4"}, {"value": "-0.92", "module": "A5"}, {"module": "B1"}, {"value": "0.0", "module": "B2"}, {"value": "0.0", "module": "B3"}, {"value": "0.0", "module": "B4"}, {"value": "0.0", "module": "B5"}, {"value": "0.0", "module": "B6"}, {"value": "0.0", "module": "B7"}, {"value": "0.0", "module": "C1"}, {"value": "0.0", "module": "C2"}, {"value": "0.0", "module": "C3"}, {"value": "0.0", "module": "C4"}, {"value": "0.0", "module": "D"}, {"name": "referenceToUnitGroupDataSet", "value": {"shortDescription": [{"value": "MJ"}], "type": "unit group data set", "refObjectId": "93a60a57-a3c8-11da-a746-0800200c9a66", "uri": "../unitgroups/93a60a57-a3c8-11da-a746-0800200c9a66"}}]}, "flowProperties": [], "typeOfFlow": "Other flow", "classification": {"classHierarchy": "Quantities", "name": "GaBiCategories"}}, {"dataSetInternalID": 16, "referenceToFlowDataSet": {"shortDescription": [{"value": "Use of renewable secondary fuels (RSF)", "lang": "en"}, {"value": "Erneuerbare Sekundärbrennstoffe (RSF)", "lang": "de"}], "type": "flow data set", "refObjectId": "64333088-a55f-4aa2-9a31-c10b07816787", "version": "38.00.000"}, "exchange direction": "INPUT", "meanAmount": 0.0, "other": {"anies": [{"value": "0.0", "module": "A1-A3"}, {"value": "0.0", "module": "A4"}, {"value": "0.0", "module": "A5"}, {"module": "B1"}, {"value": "0.0", "module": "B2"}, {"value": "0.0", "module": "B3"}, {"value": "0.0", "module": "B4"}, {"value": "0.0", "module": "B5"}, {"value": "0.0", "module": "B6"}, {"value": "0.0", "module": "B7"}, {"value": "0.0", "module": "C1"}, {"value": "0.0", "module": "C2"}, {"value": "0.0", "module": "C3"}, {"value": "0.0", "module": "C4"}, {"value": "0.0", "module": "D"}, {"name": "referenceToUnitGroupDataSet", "value": {"shortDescription": [{"value": "MJ"}], "type": "unit group data set", "refObjectId": "93a60a57-a3c8-11da-a746-0800200c9a66", "uri": "../unitgroups/93a60a57-a3c8-11da-a746-0800200c9a66"}}]}, "flowProperties": [], "typeOfFlow": "Other flow", "classification": {"classHierarchy": "Quantities / Environmental quantities / EPD EN 15804 / LCI indicators", "name": "GaBiCategories"}}, {"dataSetInternalID": 17, "referenceToFlowDataSet": {"shortDescription": [{"value": "Input of secondary material (SM)", "lang": "en"}, {"value": "Einsatz von Sekundärstoffen (SM)", "lang": "de"}], "type": "flow data set", "refObjectId": "c6a1f35f-2d09-4f54-8dfb-97e502e1ce92", "version": "38.00.000"}, "exchange direction": "INPUT", "meanAmount": 0.0, "other": {"anies": [{"value": "1.03", "module": "A1-A3"}, {"value": "0.0", "module": "A4"}, {"value": "0.0", "module": "A5"}, {"module": "B1"}, {"value": "0.0", "module": "B2"}, {"value": "0.0", "module": "B3"}, {"value": "0.0", "module": "B4"}, {"value": "1.03", "module": "B5"}, {"value": "0.0", "module": "B6"}, {"value": "0.0", "module": "B7"}, {"value": "0.0", "module": "C1"}, {"value": "0.0", "module": "C2"}, {"value": "0.0", "module": "C3"}, {"value": "0.0", "module": "C4"}, {"value": "0.0", "module": "D"}, {"name": "referenceToUnitGroupDataSet", "value": {"shortDescription": [{"value": "kg"}], "type": "unit group data set", "refObjectId": "ad38d542-3fe9-439d-9b95-2f5f7752acaf", "uri": "../unitgroups/ad38d542-3fe9-439d-9b95-2f5f7752acaf"}}]}, "flowProperties": [], "typeOfFlow": "Other flow", "classification": {"classHierarchy": "Quantities / Environmental quantities / EPD EN 15804 / LCI indicators", "name": "GaBiCategories"}}, {"dataSetInternalID": 18, "referenceToFlowDataSet": {"shortDescription": [{"value": "Total use of non-renewable primary energy resources (PENRT)", "lang": "en"}, {"value": "Total nicht erneuerbare Primärenergie (PENRT)", "lang": "de"}], "type": "flow data set", "refObjectId": "06159210-646b-4c8d-8583-da9b3b95a6c1", "version": "38.00.000"}, "exchange direction": "INPUT", "meanAmount": 0.0, "other": {"anies": [{"value": "354.11", "module": "A1-A3"}, {"value": "8.02", "module": "A4"}, {"value": "0.0219", "module": "A5"}, {"module": "B1"}, {"value": "55.2", "module": "B2"}, {"value": "0.0", "module": "B3"}, {"value": "0.0", "module": "B4"}, {"value": "283.63", "module": "B5"}, {"value": "0.0", "module": "B6"}, {"value": "0.0", "module": "B7"}, {"value": "0.0", "module": "C1"}, {"value": "2.23", "module": "C2"}, {"value": "2.62", "module": "C3"}, {"value": "0.0286", "module": "C4"}, {"value": "-89.44", "module": "D"}, {"name": "referenceToUnitGroupDataSet", "value": {"shortDescription": [{"value": "MJ"}], "type": "unit group data set", "refObjectId": "93a60a57-a3c8-11da-a746-0800200c9a66", "uri": "../unitgroups/93a60a57-a3c8-11da-a746-0800200c9a66"}}]}, "flowProperties": [], "typeOfFlow": "Other flow", "classification": {"classHierarchy": "Quantities / Environmental quantities / EPD EN 15804 / LCI indicators", "name": "GaBiCategories"}}, {"dataSetInternalID": 19, "referenceToFlowDataSet": {"shortDescription": [{"value": "Total use of renewable primary energy resources (PERT)", "lang": "en"}, {"value": "Gesamtverbrauch von erneuerbarer Primärenergie (PERT)", "lang": "de"}], "type": "flow data set", "refObjectId": "53f97275-fa8a-4cdd-9024-65936002acd0", "version": "38.00.000"}, "exchange direction": "INPUT", "meanAmount": 0.0, "other": {"anies": [{"value": "164.01", "module": "A1-A3"}, {"value": "0.68", "module": "A4"}, {"value": "0.00617", "module": "A5"}, {"module": "B1"}, {"value": "3.46", "module": "B2"}, {"value": "0.0", "module": "B3"}, {"value": "0.0", "module": "B4"}, {"value": "122.29", "module": "B5"}, {"value": "0.0", "module": "B6"}, {"value": "0.0", "module": "B7"}, {"value": "0.0", "module": "C1"}, {"value": "0.19", "module": "C2"}, {"value": "1.8", "module": "C3"}, {"value": "0.005", "module": "C4"}, {"value": "-46.46", "module": "D"}, {"name": "referenceToUnitGroupDataSet", "value": {"shortDescription": [{"value": "MJ"}], "type": "unit group data set", "refObjectId": "93a60a57-a3c8-11da-a746-0800200c9a66", "uri": "../unitgroups/93a60a57-a3c8-11da-a746-0800200c9a66"}}]}, "flowProperties": [], "typeOfFlow": "Other flow", "classification": {"classHierarchy": "Quantities / Environmental quantities / EPD EN 15804 / LCI indicators", "name": "GaBiCategories"}}]}, "LCIAResults": {"LCIAResult": [{"referenceToLCIAMethodDataSet": {"shortDescription": [{"value": "Abiotic depletion potential - non-fossil resources (ADPE)", "lang": "en"}, {"value": "Potenzial für die Verknappung abiotischer Ressourcen – nicht fossile Ressourcen (ADPE)", "lang": "de"}], "type": "LCIA method data set", "refObjectId": "b2ad6494-c78d-11e6-9d9d-cec0c932ce01", "version": "01.00.011"}, "meanAmount": 0.0, "other": {"anies": [{"value": "7.0E-6", "module": "A1-A3"}, {"value": "5.72E-8", "module": "A4"}, {"value": "1.1E-10", "module": "A5"}, {"module": "B1"}, {"value": "1.52E-7", "module": "B2"}, {"value": "0.0", "module": "B3"}, {"value": "0.0", "module": "B4"}, {"value": "4.7E-6", "module": "B5"}, {"value": "0.0", "module": "B6"}, {"value": "0.0", "module": "B7"}, {"value": "0.0", "module": "C1"}, {"value": "1.58E-8", "module": "C2"}, {"value": "2.37E-8", "module": "C3"}, {"value": "1.52E-10", "module": "C4"}, {"value": "-2.43E-6", "module": "D"}, {"name": "referenceToUnitGroupDataSet", "value": {"shortDescription": [{"value": "kg Sb-Äqv."}], "type": "unit group data set", "refObjectId": "54ccd2d9-a32a-4fc2-923d-f2c8c93e89d4", "uri": "../unitgroups/54ccd2d9-a32a-4fc2-923d-f2c8c93e89d4"}}]}}, {"referenceToLCIAMethodDataSet": {"shortDescription": [{"value": "Abiotic depletion potential - fossil resources (ADPF)", "lang": "en"}, {"value": "Potenzial für die Verknappung abiotischer Ressourcen – fossile Brennstoffe (ADPF)", "lang": "de"}], "type": "LCIA method data set", "refObjectId": "b2ad6110-c78d-11e6-9d9d-cec0c932ce01", "version": "01.00.011"}, "meanAmount": 0.0, "other": {"anies": [{"value": "389.52", "module": "A1-A3"}, {"value": "8.82", "module": "A4"}, {"value": "0.0241", "module": "A5"}, {"module": "B1"}, {"value": "60.72", "module": "B2"}, {"value": "0.0", "module": "B3"}, {"value": "0.0", "module": "B4"}, {"value": "311.99", "module": "B5"}, {"value": "0.0", "module": "B6"}, {"value": "0.0", "module": "B7"}, {"value": "0.0", "module": "C1"}, {"value": "2.45", "module": "C2"}, {"value": "2.88", "module": "C3"}, {"value": "0.0315", "module": "C4"}, {"value": "-98.38", "module": "D"}, {"name": "referenceToUnitGroupDataSet", "value": {"shortDescription": [{"value": "MJ"}], "type": "unit group data set", "refObjectId": "93a60a57-a3c8-11da-a746-0800200c9a66", "uri": "../unitgroups/93a60a57-a3c8-11da-a746-0800200c9a66"}}]}}, {"referenceToLCIAMethodDataSet": {"shortDescription": [{"value": "Acidification potential, Accumulated Exceedance (AP)", "lang": "en"}, {"value": "Versauerungspotenzial, kumulierte Überschreitung (AP)", "lang": "de"}], "type": "LCIA method data set", "refObjectId": "b5c611c6-def3-11e6-bf01-fe55135034f3", "version": "01.03.010", "uri": "http://lca.jrc.ec.europa.eu/lcainfohub/datasets/elcd/lciamethods/f6cbd466-253f-4145-a4bb-8dae7d266e89.xml"}, "meanAmount": 0.0, "other": {"anies": [{"value": "0.0854", "module": "A1-A3"}, {"value": "0.0025", "module": "A4"}, {"value": "2.13E-5", "module": "A5"}, {"module": "B1"}, {"value": "0.00256", "module": "B2"}, {"value": "0.0", "module": "B3"}, {"value": "0.0", "module": "B4"}, {"value": "0.0539", "module": "B5"}, {"value": "0.0", "module": "B6"}, {"value": "0.0", "module": "B7"}, {"value": "0.0", "module": "C1"}, {"value": "5.49E-4", "module": "C2"}, {"value": "4.53E-4", "module": "C3"}, {"value": "1.69E-5", "module": "C4"}, {"value": "-0.0354", "module": "D"}, {"name": "referenceToUnitGroupDataSet", "value": {"shortDescription": [{"value": "mol H+ eqv."}], "type": "unit group data set", "refObjectId": "42e089ac-92bf-4bf2-8ca1-5fc40d18f2ed", "uri": "../unitgroups/42e089ac-92bf-4bf2-8ca1-5fc40d18f2ed"}}]}}, {"referenceToLCIAMethodDataSet": {"shortDescription": [{"value": "Eutrophication potential - freshwater (EP-freshwater)", "lang": "en"}, {"value": "Eutrophierungspotenzial - Süßwasser (EP-freshwater)", "lang": "de"}], "type": "LCIA method data set", "refObjectId": "b53ec18f-7377-4ad3-86eb-cc3f4f276b2b", "version": "01.00.011", "uri": "http://lca.jrc.ec.europa.eu/lcainfohub/datasets/elcd/lciamethods/a4630d5b-df2f-48ae-b3f2-5e5257606d68.xml"}, "meanAmount": 0.0, "other": {"anies": [{"value": "1.21E-4", "module": "A1-A3"}, {"value": "2.88E-6", "module": "A4"}, {"value": "2.74E-9", "module": "A5"}, {"module": "B1"}, {"value": "3.42E-6", "module": "B2"}, {"value": "0.0", "module": "B3"}, {"value": "0.0", "module": "B4"}, {"value": "1.22E-4", "module": "B5"}, {"value": "0.0", "module": "B6"}, {"value": "0.0", "module": "B7"}, {"value": "0.0", "module": "C1"}, {"value": "8.02E-7", "module": "C2"}, {"value": "5.46E-7", "module": "C3"}, {"value": "5.42E-9", "module": "C4"}, {"value": "-4.15E-6", "module": "D"}, {"name": "referenceToUnitGroupDataSet", "value": {"shortDescription": [{"value": "kg P eqv."}], "type": "unit group data set", "refObjectId": "0429039d-a61d-4590-ba67-aa4a20a810a1", "uri": "../unitgroups/0429039d-a61d-4590-ba67-aa4a20a810a1"}}]}}, {"referenceToLCIAMethodDataSet": {"shortDescription": [{"value": "Eutrophication potential - marine (EP-marine)", "lang": "en"}, {"value": "Eutrophierungspotenzial - Salzwasser (EP-marine)", "lang": "de"}], "type": "LCIA method data set", "refObjectId": "b5c619fa-def3-11e6-bf01-fe55135034f3", "version": "02.00.011", "uri": "http://lca.jrc.ec.europa.eu/lcainfohub/datasets/elcd/lciamethods/5296e2be-060b-4e50-b033-d45f85f6ac92.xml"}, "meanAmount": 0.0, "other": {"anies": [{"value": "0.0226", "module": "A1-A3"}, {"value": "0.00116", "module": "A4"}, {"value": "6.34E-6", "module": "A5"}, {"module": "B1"}, {"value": "8.05E-4", "module": "B2"}, {"value": "0.0", "module": "B3"}, {"value": "0.0", "module": "B4"}, {"value": "0.0171", "module": "B5"}, {"value": "0.0", "module": "B6"}, {"value": "0.0", "module": "B7"}, {"value": "0.0", "module": "C1"}, {"value": "2.48E-4", "module": "C2"}, {"value": "1.06E-4", "module": "C3"}, {"value": "4.37E-6", "module": "C4"}, {"value": "-0.00706", "module": "D"}, {"name": "referenceToUnitGroupDataSet", "value": {"shortDescription": [{"value": "kg N eqv."}], "type": "unit group data set", "refObjectId": "d05bb823-ecdf-4686-8c40-bf1d9257859f", "uri": "../unitgroups/d05bb823-ecdf-4686-8c40-bf1d9257859f"}}]}}, {"referenceToLCIAMethodDataSet": {"shortDescription": [{"value": "Eutrophication potential - terrestrial (EP-terrestrial)", "lang": "en"}, {"value": "Eutrophierungspotenzial - Land (EP-terrestrial)", "lang": "de"}], "type": "LCIA method data set", "refObjectId": "b5c614d2-def3-11e6-bf01-fe55135034f3", "version": "01.02.010", "uri": "http://lca.jrc.ec.europa.eu/lcainfohub/datasets/elcd/lciamethods/40054970-5936-477c-9bec-29fa23b1cb77.xml"}, "meanAmount": 0.0, "other": {"anies": [{"value": "0.2", "module": "A1-A3"}, {"value": "0.013", "module": "A4"}, {"value": "9.93E-5", "module": "A5"}, {"module": "B1"}, {"value": "0.00873", "module": "B2"}, {"value": "0.0", "module": "B3"}, {"value": "0.0", "module": "B4"}, {"value": "0.14", "module": "B5"}, {"value": "0.0", "module": "B6"}, {"value": "0.0", "module": "B7"}, {"value": "0.0", "module": "C1"}, {"value": "0.00279", "module": "C2"}, {"value": "0.00163", "module": "C3"}, {"value": "4.81E-5", "module": "C4"}, {"value": "-0.0773", "module": "D"}, {"name": "referenceToUnitGroupDataSet", "value": {"shortDescription": [{"value": "mol N eqv."}], "type": "unit group data set", "refObjectId": "71b4d617-0ec9-4d3f-b65e-e438940c2401", "uri": "../unitgroups/71b4d617-0ec9-4d3f-b65e-e438940c2401"}}]}}, {"referenceToLCIAMethodDataSet": {"shortDescription": [{"value": "Global Warming Potential - total (GWP-total)", "lang": "en"}, {"value": "Globales Erwärmungspotenzial - total (GWP-total)", "lang": "de"}], "type": "LCIA method data set", "refObjectId": "6a37f984-a4b3-458a-a20a-64418c145fa2", "version": "04.00.017"}, "meanAmount": 0.0, "other": {"anies": [{"value": "27.24", "module": "A1-A3"}, {"value": "0.69", "module": "A4"}, {"value": "0.14", "module": "A5"}, {"module": "B1"}, {"value": "3.07", "module": "B2"}, {"value": "0.0", "module": "B3"}, {"value": "0.0", "module": "B4"}, {"value": "23.06", "module": "B5"}, {"value": "0.0", "module": "B6"}, {"value": "0.0", "module": "B7"}, {"value": "0.0", "module": "C1"}, {"value": "0.19", "module": "C2"}, {"value": "2.23", "module": "C3"}, {"value": "0.00244", "module": "C4"}, {"value": "-7.83", "module": "D"}, {"name": "referenceToUnitGroupDataSet", "value": {"shortDescription": [{"value": "kg CO2-Äqv."}], "type": "unit group data set", "refObjectId": "1ebf3012-d0db-4de2-aefd-ef30cedb0be1", "uri": "../unitgroups/1ebf3012-d0db-4de2-aefd-ef30cedb0be1"}}]}}, {"referenceToLCIAMethodDataSet": {"shortDescription": [{"value": "Global Warming Potential - fossil fuels (GWP-fossil)", "lang": "en"}, {"value": "Globales Erwärmungspotenzial - fossil (GWP-fossil)", "lang": "de"}], "type": "LCIA method data set", "refObjectId": "5f635281-343e-44fb-83df-1971b155e6b6", "version": "01.00.009"}, "meanAmount": 0.0, "other": {"anies": [{"value": "27.07", "module": "A1-A3"}, {"value": "0.7", "module": "A4"}, {"value": "0.0999", "module": "A5"}, {"module": "B1"}, {"value": "3.06", "module": "B2"}, {"value": "0.0", "module": "B3"}, {"value": "0.0", "module": "B4"}, {"value": "22.87", "module": "B5"}, {"value": "0.0", "module": "B6"}, {"value": "0.0", "module": "B7"}, {"value": "0.0", "module": "C1"}, {"value": "0.19", "module": "C2"}, {"value": "2.23", "module": "C3"}, {"value": "0.00244", "module": "C4"}, {"value": "-7.8", "module": "D"}, {"name": "referenceToUnitGroupDataSet", "value": {"shortDescription": [{"value": "kg CO2-Äqv."}], "type": "unit group data set", "refObjectId": "1ebf3012-d0db-4de2-aefd-ef30cedb0be1", "uri": "../unitgroups/1ebf3012-d0db-4de2-aefd-ef30cedb0be1"}}]}}, {"referenceToLCIAMethodDataSet": {"shortDescription": [{"value": "Global Warming Potential - biogenic (GWP-biogenic)", "lang": "en"}, {"value": "Globales Erwärmungspotenzial - biogen (GWP-biogenic)", "lang": "de"}], "type": "LCIA method data set", "refObjectId": "2356e1ab-0185-4db5-86e5-16de51c7485c", "version": "01.00.006"}, "meanAmount": 0.0, "other": {"anies": [{"value": "0.17", "module": "A1-A3"}, {"value": "-0.0154", "module": "A4"}, {"value": "0.0367", "module": "A5"}, {"module": "B1"}, {"value": "0.012", "module": "B2"}, {"value": "0.0", "module": "B3"}, {"value": "0.0", "module": "B4"}, {"value": "0.16", "module": "B5"}, {"value": "0.0", "module": "B6"}, {"value": "0.0", "module": "B7"}, {"value": "0.0", "module": "C1"}, {"value": "-0.00428", "module": "C2"}, {"value": "0.00136", "module": "C3"}, {"value": "-1.33E-5", "module": "C4"}, {"value": "-0.023", "module": "D"}, {"name": "referenceToUnitGroupDataSet", "value": {"shortDescription": [{"value": "kg CO2-Äqv."}], "type": "unit group data set", "refObjectId": "1ebf3012-d0db-4de2-aefd-ef30cedb0be1", "uri": "../unitgroups/1ebf3012-d0db-4de2-aefd-ef30cedb0be1"}}]}}, {"referenceToLCIAMethodDataSet": {"shortDescription": [{"value": "Global Warming Potential - land use and land use change (GWP-luluc)", "lang": "en"}, {"value": "Globales Erwärmungspotenzial - luluc (GWP-luluc)", "lang": "de"}], "type": "LCIA method data set", "refObjectId": "4331bbdb-978a-490d-8707-eeb047f01a55", "version": "01.00.006"}, "meanAmount": 0.0, "other": {"anies": [{"value": "0.00652", "module": "A1-A3"}, {"value": "0.0113", "module": "A4"}, {"value": "8.34E-7", "module": "A5"}, {"module": "B1"}, {"value": "4.31E-4", "module": "B2"}, {"value": "0.0", "module": "B3"}, {"value": "0.0", "module": "B4"}, {"value": "0.0196", "module": "B5"}, {"value": "0.0", "module": "B6"}, {"value": "0.0", "module": "B7"}, {"value": "0.0", "module": "C1"}, {"value": "0.00316", "module": "C2"}, {"value": "2.33E-5", "module": "C3"}, {"value": "1.43E-5", "module": "C4"}, {"value": "-0.00145", "module": "D"}, {"name": "referenceToUnitGroupDataSet", "value": {"shortDescription": [{"value": "kg CO2-Äqv."}], "type": "unit group data set", "refObjectId": "1ebf3012-d0db-4de2-aefd-ef30cedb0be1", "uri": "../unitgroups/1ebf3012-d0db-4de2-aefd-ef30cedb0be1"}}]}}, {"referenceToLCIAMethodDataSet": {"shortDescription": [{"value": "Depletion potential of the stratospheric ozone layer (ODP)", "lang": "en"}, {"value": "Abbaupotenzial der stratosphärischen Ozonschicht (ODP)", "lang": "de"}], "type": "LCIA method data set", "refObjectId": "b5c629d6-def3-11e6-bf01-fe55135034f3", "version": "02.00.013", "uri": "http://lca.jrc.ec.europa.eu/lcainfohub/datasets/elcd/lciamethods/8b723200-3d8f-4eec-9e10-444edb029476.xml"}, "meanAmount": 0.0, "other": {"anies": [{"value": "1.11E-8", "module": "A1-A3"}, {"value": "6.81E-14", "module": "A4"}, {"value": "1.09E-14", "module": "A5"}, {"module": "B1"}, {"value": "7.67E-12", "module": "B2"}, {"value": "0.0", "module": "B3"}, {"value": "0.0", "module": "B4"}, {"value": "1.11E-8", "module": "B5"}, {"value": "0.0", "module": "B6"}, {"value": "0.0", "module": "B7"}, {"value": "0.0", "module": "C1"}, {"value": "1.89E-14", "module": "C2"}, {"value": "2.96E-12", "module": "C3"}, {"value": "6.45E-15", "module": "C4"}, {"value": "-1.62E-11", "module": "D"}, {"name": "referenceToUnitGroupDataSet", "value": {"shortDescription": [{"value": "kg CFC 11-Äquiv."}], "type": "unit group data set", "refObjectId": "d9e957c9-7309-4474-bf3a-7777df6c4e5b", "uri": "../unitgroups/d9e957c9-7309-4474-bf3a-7777df6c4e5b"}}]}}, {"referenceToLCIAMethodDataSet": {"shortDescription": [{"value": "Photochemical Ozone Creation Potential (POCP)", "lang": "en"}, {"value": "Bildungspotenzial für troposphärisches Ozon (POCP)", "lang": "de"}], "type": "LCIA method data set", "refObjectId": "b5c610fe-def3-11e6-bf01-fe55135034f3", "version": "02.00.015", "uri": "http://lca.jrc.ec.europa.eu/lcainfohub/datasets/elcd/lciamethods/ec7836be-83eb-41da-bcda-1a6a3fe2d149.xml"}, "meanAmount": 0.0, "other": {"anies": [{"value": "0.0535", "module": "A1-A3"}, {"value": "0.00237", "module": "A4"}, {"value": "1.75E-5", "module": "A5"}, {"module": "B1"}, {"value": "0.00364", "module": "B2"}, {"value": "0.0", "module": "B3"}, {"value": "0.0", "module": "B4"}, {"value": "0.0362", "module": "B5"}, {"value": "0.0", "module": "B6"}, {"value": "0.0", "module": "B7"}, {"value": "0.0", "module": "C1"}, {"value": "5.2E-4", "module": "C2"}, {"value": "2.95E-4", "module": "C3"}, {"value": "1.33E-5", "module": "C4"}, {"value": "-0.0208", "module": "D"}, {"name": "referenceToUnitGroupDataSet", "value": {"shortDescription": [{"value": "kg NMVOC eqv."}], "type": "unit group data set", "refObjectId": "d27c25f8-fbc1-44c6-b47b-4adbae4199c6", "uri": "../unitgroups/d27c25f8-fbc1-44c6-b47b-4adbae4199c6"}}]}}, {"referenceToLCIAMethodDataSet": {"shortDescription": [{"value": "Water (user) deprivation potential (WDP)", "lang": "en"}, {"value": "Wasser-Entzugspotenzial (Benutzer) (WDP)", "lang": "de"}], "type": "LCIA method data set", "refObjectId": "b2ad66ce-c78d-11e6-9d9d-cec0c932ce01", "version": "03.00.015"}, "meanAmount": 0.0, "other": {"anies": [{"value": "6.74", "module": "A1-A3"}, {"value": "0.0101", "module": "A4"}, {"value": "0.0143", "module": "A5"}, {"module": "B1"}, {"value": "0.24", "module": "B2"}, {"value": "0.0", "module": "B3"}, {"value": "0.0", "module": "B4"}, {"value": "4.22", "module": "B5"}, {"value": "0.0", "module": "B6"}, {"value": "0.0", "module": "B7"}, {"value": "0.0", "module": "C1"}, {"value": "0.00279", "module": "C2"}, {"value": "0.23", "module": "C3"}, {"value": "2.73E-4", "module": "C4"}, {"value": "-2.82", "module": "D"}, {"name": "referenceToUnitGroupDataSet", "value": {"shortDescription": [{"value": "m3 world eqv."}], "type": "unit group data set", "refObjectId": "6ae2df01-888e-46c8-b17d-49fa3869b476", "uri": "../unitgroups/6ae2df01-888e-46c8-b17d-49fa3869b476"}}]}}, {"referenceToLCIAMethodDataSet": {"shortDescription": [{"value": "Potential incidence of disease due to PM emissions (PM)", "lang": "en"}, {"value": "Potenzielles Auftreten von Krankheiten aufgrund von Feinstaubemissionen (PM)", "lang": "de"}], "type": "LCIA method data set", "refObjectId": "b5c602c6-def3-11e6-bf01-fe55135034f3", "version": "02.00.012", "uri": "http://lca.jrc.ec.europa.eu/lcainfohub/datasets/elcd/lciamethods/72ce3013-f678-4c6a-935b-f4752ff8901b.xml"}, "meanAmount": 0.0, "other": {"anies": [{"value": "1.34E-6", "module": "A1-A3"}, {"value": "1.91E-8", "module": "A4"}, {"value": "1.21E-10", "module": "A5"}, {"module": "B1"}, {"value": "2.13E-8", "module": "B2"}, {"value": "0.0", "module": "B3"}, {"value": "0.0", "module": "B4"}, {"value": "7.25E-7", "module": "B5"}, {"value": "0.0", "module": "B6"}, {"value": "0.0", "module": "B7"}, {"value": "0.0", "module": "C1"}, {"value": "4.21E-9", "module": "C2"}, {"value": "3.26E-9", "module": "C3"}, {"value": "2.12E-10", "module": "C4"}, {"value": "-6.48E-7", "module": "D"}, {"name": "referenceToUnitGroupDataSet", "value": {"shortDescription": [{"value": "disease incidence"}], "type": "unit group data set", "refObjectId": "3883559b-648f-4afc-8ba2-0bd24f3affa3", "uri": "../unitgroups/3883559b-648f-4afc-8ba2-0bd24f3affa3"}}]}}, {"referenceToLCIAMethodDataSet": {"shortDescription": [{"value": "Potential Human exposure efficiency relative to U235 (IRP)", "lang": "en"}, {"value": "Potenzielle Wirkung durch Exposition des Menschen mit U235 (IRP)", "lang": "de"}], "type": "LCIA method data set", "refObjectId": "b5c632be-def3-11e6-bf01-fe55135034f3", "version": "01.00.012", "uri": "http://lca.jrc.ec.europa.eu/lcainfohub/datasets/elcd/lciamethods/a6f4cbc8-5388-44d6-9a67-53d05684f93e.xml"}, "meanAmount": 0.0, "other": {"anies": [{"value": "1.75", "module": "A1-A3"}, {"value": "0.0016", "module": "A4"}, {"value": "2.06E-4", "module": "A5"}, {"module": "B1"}, {"value": "0.0455", "module": "B2"}, {"value": "0.0", "module": "B3"}, {"value": "0.0", "module": "B4"}, {"value": "1.27", "module": "B5"}, {"value": "0.0", "module": "B6"}, {"value": "0.0", "module": "B7"}, {"value": "0.0", "module": "C1"}, {"value": "4.42E-4", "module": "C2"}, {"value": "0.0717", "module": "C3"}, {"value": "3.83E-5", "module": "C4"}, {"value": "-0.64", "module": "D"}, {"name": "referenceToUnitGroupDataSet", "value": {"shortDescription": [{"value": "kBq U235 eqv."}], "type": "unit group data set", "refObjectId": "456b05bf-1415-44a9-9993-02452f554c09", "uri": "../unitgroups/456b05bf-1415-44a9-9993-02452f554c09"}}]}}, {"referenceToLCIAMethodDataSet": {"shortDescription": [{"value": "Potential Comparative Toxic Unit for ecosystems (ETP-fw)", "lang": "en"}, {"value": "Potenzielle Toxizitätsvergleichseinheit für Ökosysteme (ETP-fw)", "lang": "de"}], "type": "LCIA method data set", "refObjectId": "ee1082d1-b0f7-43ca-a1f0-21e2a4a74511", "version": "01.00.003", "uri": "http://lca.jrc.ec.europa.eu/lcainfohub/datasets/elcd/lciamethods/ee1082d1-b0f7-43ca-a1f0-21e2a4a74511.xml"}, "meanAmount": 0.0, "other": {"anies": [{"value": "849.28", "module": "A1-A3"}, {"value": "6.42", "module": "A4"}, {"value": "0.0117", "module": "A5"}, {"module": "B1"}, {"value": "26.29", "module": "B2"}, {"value": "0.0", "module": "B3"}, {"value": "0.0", "module": "B4"}, {"value": "818.58", "module": "B5"}, {"value": "0.0", "module": "B6"}, {"value": "0.0", "module": "B7"}, {"value": "0.0", "module": "C1"}, {"value": "1.78", "module": "C2"}, {"value": "1.32", "module": "C3"}, {"value": "0.0183", "module": "C4"}, {"value": "-41.75", "module": "D"}, {"name": "referenceToUnitGroupDataSet", "value": {"shortDescription": [{"value": "CTUe"}], "type": "unit group data set", "refObjectId": "aa959ded-f1eb-4efb-9c5c-2d60be36b3e6", "uri": "../unitgroups/aa959ded-f1eb-4efb-9c5c-2d60be36b3e6"}}]}}, {"referenceToLCIAMethodDataSet": {"shortDescription": [{"value": "Potential Comparative Toxic Unit for humans - cancer effects (HTP-c)", "lang": "en"}, {"value": "Potenzielle Toxizitätsvergleichseinheit für den Menschen - kanzerogene Wirkung (HTP-c)", "lang": "de"}], "type": "LCIA method data set", "refObjectId": "2299222a-bbd8-474f-9d4f-4dd1f18aea7c", "version": "01.00.004", "uri": "http://lca.jrc.ec.europa.eu/lcainfohub/datasets/elcd/lciamethods/2299222a-bbd8-474f-9d4f-4dd1f18aea7c.xml"}, "meanAmount": 0.0, "other": {"anies": [{"value": "6.36E-8", "module": "A1-A3"}, {"value": "1.31E-10", "module": "A4"}, {"value": "9.75E-13", "module": "A5"}, {"module": "B1"}, {"value": "6.58E-10", "module": "B2"}, {"value": "0.0", "module": "B3"}, {"value": "0.0", "module": "B4"}, {"value": "2.87E-8", "module": "B5"}, {"value": "0.0", "module": "B6"}, {"value": "0.0", "module": "B7"}, {"value": "0.0", "module": "C1"}, {"value": "3.63E-11", "module": "C2"}, {"value": "5.67E-11", "module": "C3"}, {"value": "4.28E-13", "module": "C4"}, {"value": "-3.52E-8", "module": "D"}, {"name": "referenceToUnitGroupDataSet", "value": {"shortDescription": [{"value": "CTUh"}], "type": "unit group data set", "refObjectId": "d4c9523e-2d7e-49fd-8469-998f547d3a70", "uri": "../unitgroups/d4c9523e-2d7e-49fd-8469-998f547d3a70"}}]}}, {"referenceToLCIAMethodDataSet": {"shortDescription": [{"value": "Potential Comparative Toxic Unit for humans - non-cancer effects (HTP-nc)", "lang": "en"}, {"value": "Potenzielle Toxizitätsvergleichseinheit für den Menschen - nicht kanzerogene Wirkung (HTP-nc)", "lang": "de"}], "type": "LCIA method data set", "refObjectId": "3af763a5-b7a1-48c9-9cee-1f223481fcef", "version": "01.00.003", "uri": "http://lca.jrc.ec.europa.eu/lcainfohub/datasets/elcd/lciamethods/3af763a5-b7a1-48c9-9cee-1f223481fcef.xml"}, "meanAmount": 0.0, "other": {"anies": [{"value": "2.26E-7", "module": "A1-A3"}, {"value": "7.73E-9", "module": "A4"}, {"value": "3.04E-11", "module": "A5"}, {"module": "B1"}, {"value": "3.25E-8", "module": "B2"}, {"value": "0.0", "module": "B3"}, {"value": "0.0", "module": "B4"}, {"value": "1.67E-7", "module": "B5"}, {"value": "0.0", "module": "B6"}, {"value": "0.0", "module": "B7"}, {"value": "0.0", "module": "C1"}, {"value": "2.1E-9", "module": "C2"}, {"value": "1.39E-9", "module": "C3"}, {"value": "2.83E-11", "module": "C4"}, {"value": "-7.22E-8", "module": "D"}, {"name": "referenceToUnitGroupDataSet", "value": {"shortDescription": [{"value": "CTUh"}], "type": "unit group data set", "refObjectId": "d4c9523e-2d7e-49fd-8469-998f547d3a70", "uri": "../unitgroups/d4c9523e-2d7e-49fd-8469-998f547d3a70"}}]}}, {"referenceToLCIAMethodDataSet": {"shortDescription": [{"value": "Potential Soil quality index (SQP)", "lang": "en"}, {"value": "Potenzieller Bodenqualitätsindex (SQP)", "lang": "de"}], "type": "LCIA method data set", "refObjectId": "b2ad6890-c78d-11e6-9d9d-cec0c932ce01", "version": "01.00.011"}, "meanAmount": 0.0, "other": {"anies": [{"value": "85.64", "module": "A1-A3"}, {"value": "4.37", "module": "A4"}, {"value": "0.00758", "module": "A5"}, {"module": "B1"}, {"value": "2.67", "module": "B2"}, {"value": "0.0", "module": "B3"}, {"value": "0.0", "module": "B4"}, {"value": "86.7", "module": "B5"}, {"value": "0.0", "module": "B6"}, {"value": "0.0", "module": "B7"}, {"value": "0.0", "module": "C1"}, {"value": "1.21", "module": "C2"}, {"value": "1.19", "module": "C3"}, {"value": "0.00867", "module": "C4"}, {"value": "-7.04", "module": "D"}, {"name": "referenceToUnitGroupDataSet", "value": {"shortDescription": [{"value": "dimensionless"}], "type": "unit group data set", "refObjectId": "f130951c-e67f-4f7f-8dd4-665de3974e18", "uri": "../unitgroups/f130951c-e67f-4f7f-8dd4-665de3974e18"}}]}}]}, "otherAttributes": {"{http://www.okworx.com/ILCD/Extensions/2018/Profile}profile": "EN_15804_A2", "{http://www.indata.network/EPD/2019}epd-version": "1.2"}, "version": "1.1"}