{"processInformation": {"dataSetInformation": {"UUID": "263ce306-f149-4dbd-9a5d-72281d46dbac", "name": {"baseName": [{"value": "Flachdachfenster - Roto Frank DST - Flachdachfenster OnTop Fixverglast (FF Fi)", "lang": "de"}, {"value": "flat roof window - Roto Frank DST - flat roof window OnTop Fixed glazed (FF Fi)", "lang": "en"}]}, "classificationInformation": {"classification": [{"class": [{"value": "Komponenten von Fenstern und Vorhangfassaden", "level": 0, "classId": "7"}, {"value": "Tageslichtsysteme und Rauch- / Wärmeabzugsanlagen ", "level": 1, "classId": "7.10"}, {"value": "Oberlichter", "level": 2, "classId": "7.10.01"}], "name": "OEKOBAU.DAT"}]}, "generalComment": [{"value": "Dieser Datensatz beinhaltet die Ergebnisse für die Module A1-A3 sowie Module A4, A5, B1, B2, B3, B4, B5, B6, B7, C1, C2, C3, C4, D. Das Umweltprofil beinhaltet die Aufwendungen für die Lebenszyklus-Stadien cradle to grave (Modul A + B + C + D). Die Herstellung der Verpackung wurde innerhalb der Module A1-A3 berücksichtigt.", "lang": "de"}, {"value": "This data set contains the results for modules A1-A3 and modules A4, A5, B1, B2, B3, B4, B5, B6, B7, C1, C2, C3, C4, D. The environmental profile contains the expenditure for the cradle to grave life cycle stages (modules A + B + C + D). The production of the packaging was taken into account within modules A1-A3.", "lang": "en"}], "other": {"anies": [{"margins": 0.0}, "<ns11:modules xmlns:ns11=\"http://openlca.org/epd_ilcd\" xmlns=\"http://lca.jrc.it/ILCD/Process\" xmlns:c=\"http://lca.jrc.it/ILCD/Contact\" xmlns:common=\"http://lca.jrc.it/ILCD/Common\" xmlns:epd=\"http://www.iai.kit.edu/EPD/2013\" xmlns:epd2=\"http://www.indata.network/EPD/2019\" xmlns:f=\"http://lca.jrc.it/ILCD/Flow\" xmlns:fp=\"http://lca.jrc.it/ILCD/FlowProperty\" xmlns:m=\"http://lca.jrc.it/ILCD/LCIAMethod\" xmlns:ns9=\"http://www.okworx.com/ILCD/Extensions/2018/Profile\" xmlns:s=\"http://lca.jrc.it/ILCD/Source\" xmlns:u=\"http://lca.jrc.it/ILCD/UnitGroup\" name=\"A1-A3\"/>", "<ns11:modules xmlns:ns11=\"http://openlca.org/epd_ilcd\" xmlns=\"http://lca.jrc.it/ILCD/Process\" xmlns:c=\"http://lca.jrc.it/ILCD/Contact\" xmlns:common=\"http://lca.jrc.it/ILCD/Common\" xmlns:epd=\"http://www.iai.kit.edu/EPD/2013\" xmlns:epd2=\"http://www.indata.network/EPD/2019\" xmlns:f=\"http://lca.jrc.it/ILCD/Flow\" xmlns:fp=\"http://lca.jrc.it/ILCD/FlowProperty\" xmlns:m=\"http://lca.jrc.it/ILCD/LCIAMethod\" xmlns:ns9=\"http://www.okworx.com/ILCD/Extensions/2018/Profile\" xmlns:s=\"http://lca.jrc.it/ILCD/Source\" xmlns:u=\"http://lca.jrc.it/ILCD/UnitGroup\" name=\"A4\"/>", "<ns11:modules xmlns:ns11=\"http://openlca.org/epd_ilcd\" xmlns=\"http://lca.jrc.it/ILCD/Process\" xmlns:c=\"http://lca.jrc.it/ILCD/Contact\" xmlns:common=\"http://lca.jrc.it/ILCD/Common\" xmlns:epd=\"http://www.iai.kit.edu/EPD/2013\" xmlns:epd2=\"http://www.indata.network/EPD/2019\" xmlns:f=\"http://lca.jrc.it/ILCD/Flow\" xmlns:fp=\"http://lca.jrc.it/ILCD/FlowProperty\" xmlns:m=\"http://lca.jrc.it/ILCD/LCIAMethod\" xmlns:ns9=\"http://www.okworx.com/ILCD/Extensions/2018/Profile\" xmlns:s=\"http://lca.jrc.it/ILCD/Source\" xmlns:u=\"http://lca.jrc.it/ILCD/UnitGroup\" name=\"A5\"/>", "<ns11:modules xmlns:ns11=\"http://openlca.org/epd_ilcd\" xmlns=\"http://lca.jrc.it/ILCD/Process\" xmlns:c=\"http://lca.jrc.it/ILCD/Contact\" xmlns:common=\"http://lca.jrc.it/ILCD/Common\" xmlns:epd=\"http://www.iai.kit.edu/EPD/2013\" xmlns:epd2=\"http://www.indata.network/EPD/2019\" xmlns:f=\"http://lca.jrc.it/ILCD/Flow\" xmlns:fp=\"http://lca.jrc.it/ILCD/FlowProperty\" xmlns:m=\"http://lca.jrc.it/ILCD/LCIAMethod\" xmlns:ns9=\"http://www.okworx.com/ILCD/Extensions/2018/Profile\" xmlns:s=\"http://lca.jrc.it/ILCD/Source\" xmlns:u=\"http://lca.jrc.it/ILCD/UnitGroup\" name=\"B1\"/>", "<ns11:modules xmlns:ns11=\"http://openlca.org/epd_ilcd\" xmlns=\"http://lca.jrc.it/ILCD/Process\" xmlns:c=\"http://lca.jrc.it/ILCD/Contact\" xmlns:common=\"http://lca.jrc.it/ILCD/Common\" xmlns:epd=\"http://www.iai.kit.edu/EPD/2013\" xmlns:epd2=\"http://www.indata.network/EPD/2019\" xmlns:f=\"http://lca.jrc.it/ILCD/Flow\" xmlns:fp=\"http://lca.jrc.it/ILCD/FlowProperty\" xmlns:m=\"http://lca.jrc.it/ILCD/LCIAMethod\" xmlns:ns9=\"http://www.okworx.com/ILCD/Extensions/2018/Profile\" xmlns:s=\"http://lca.jrc.it/ILCD/Source\" xmlns:u=\"http://lca.jrc.it/ILCD/UnitGroup\" name=\"B2\"/>", "<ns11:modules xmlns:ns11=\"http://openlca.org/epd_ilcd\" xmlns=\"http://lca.jrc.it/ILCD/Process\" xmlns:c=\"http://lca.jrc.it/ILCD/Contact\" xmlns:common=\"http://lca.jrc.it/ILCD/Common\" xmlns:epd=\"http://www.iai.kit.edu/EPD/2013\" xmlns:epd2=\"http://www.indata.network/EPD/2019\" xmlns:f=\"http://lca.jrc.it/ILCD/Flow\" xmlns:fp=\"http://lca.jrc.it/ILCD/FlowProperty\" xmlns:m=\"http://lca.jrc.it/ILCD/LCIAMethod\" xmlns:ns9=\"http://www.okworx.com/ILCD/Extensions/2018/Profile\" xmlns:s=\"http://lca.jrc.it/ILCD/Source\" xmlns:u=\"http://lca.jrc.it/ILCD/UnitGroup\" name=\"B3\"/>", "<ns11:modules xmlns:ns11=\"http://openlca.org/epd_ilcd\" xmlns=\"http://lca.jrc.it/ILCD/Process\" xmlns:c=\"http://lca.jrc.it/ILCD/Contact\" xmlns:common=\"http://lca.jrc.it/ILCD/Common\" xmlns:epd=\"http://www.iai.kit.edu/EPD/2013\" xmlns:epd2=\"http://www.indata.network/EPD/2019\" xmlns:f=\"http://lca.jrc.it/ILCD/Flow\" xmlns:fp=\"http://lca.jrc.it/ILCD/FlowProperty\" xmlns:m=\"http://lca.jrc.it/ILCD/LCIAMethod\" xmlns:ns9=\"http://www.okworx.com/ILCD/Extensions/2018/Profile\" xmlns:s=\"http://lca.jrc.it/ILCD/Source\" xmlns:u=\"http://lca.jrc.it/ILCD/UnitGroup\" name=\"B4\"/>", "<ns11:modules xmlns:ns11=\"http://openlca.org/epd_ilcd\" xmlns=\"http://lca.jrc.it/ILCD/Process\" xmlns:c=\"http://lca.jrc.it/ILCD/Contact\" xmlns:common=\"http://lca.jrc.it/ILCD/Common\" xmlns:epd=\"http://www.iai.kit.edu/EPD/2013\" xmlns:epd2=\"http://www.indata.network/EPD/2019\" xmlns:f=\"http://lca.jrc.it/ILCD/Flow\" xmlns:fp=\"http://lca.jrc.it/ILCD/FlowProperty\" xmlns:m=\"http://lca.jrc.it/ILCD/LCIAMethod\" xmlns:ns9=\"http://www.okworx.com/ILCD/Extensions/2018/Profile\" xmlns:s=\"http://lca.jrc.it/ILCD/Source\" xmlns:u=\"http://lca.jrc.it/ILCD/UnitGroup\" name=\"B5\"/>", "<ns11:modules xmlns:ns11=\"http://openlca.org/epd_ilcd\" xmlns=\"http://lca.jrc.it/ILCD/Process\" xmlns:c=\"http://lca.jrc.it/ILCD/Contact\" xmlns:common=\"http://lca.jrc.it/ILCD/Common\" xmlns:epd=\"http://www.iai.kit.edu/EPD/2013\" xmlns:epd2=\"http://www.indata.network/EPD/2019\" xmlns:f=\"http://lca.jrc.it/ILCD/Flow\" xmlns:fp=\"http://lca.jrc.it/ILCD/FlowProperty\" xmlns:m=\"http://lca.jrc.it/ILCD/LCIAMethod\" xmlns:ns9=\"http://www.okworx.com/ILCD/Extensions/2018/Profile\" xmlns:s=\"http://lca.jrc.it/ILCD/Source\" xmlns:u=\"http://lca.jrc.it/ILCD/UnitGroup\" name=\"B6\"/>", "<ns11:modules xmlns:ns11=\"http://openlca.org/epd_ilcd\" xmlns=\"http://lca.jrc.it/ILCD/Process\" xmlns:c=\"http://lca.jrc.it/ILCD/Contact\" xmlns:common=\"http://lca.jrc.it/ILCD/Common\" xmlns:epd=\"http://www.iai.kit.edu/EPD/2013\" xmlns:epd2=\"http://www.indata.network/EPD/2019\" xmlns:f=\"http://lca.jrc.it/ILCD/Flow\" xmlns:fp=\"http://lca.jrc.it/ILCD/FlowProperty\" xmlns:m=\"http://lca.jrc.it/ILCD/LCIAMethod\" xmlns:ns9=\"http://www.okworx.com/ILCD/Extensions/2018/Profile\" xmlns:s=\"http://lca.jrc.it/ILCD/Source\" xmlns:u=\"http://lca.jrc.it/ILCD/UnitGroup\" name=\"B7\"/>", "<ns11:modules xmlns:ns11=\"http://openlca.org/epd_ilcd\" xmlns=\"http://lca.jrc.it/ILCD/Process\" xmlns:c=\"http://lca.jrc.it/ILCD/Contact\" xmlns:common=\"http://lca.jrc.it/ILCD/Common\" xmlns:epd=\"http://www.iai.kit.edu/EPD/2013\" xmlns:epd2=\"http://www.indata.network/EPD/2019\" xmlns:f=\"http://lca.jrc.it/ILCD/Flow\" xmlns:fp=\"http://lca.jrc.it/ILCD/FlowProperty\" xmlns:m=\"http://lca.jrc.it/ILCD/LCIAMethod\" xmlns:ns9=\"http://www.okworx.com/ILCD/Extensions/2018/Profile\" xmlns:s=\"http://lca.jrc.it/ILCD/Source\" xmlns:u=\"http://lca.jrc.it/ILCD/UnitGroup\" name=\"C1\"/>", "<ns11:modules xmlns:ns11=\"http://openlca.org/epd_ilcd\" xmlns=\"http://lca.jrc.it/ILCD/Process\" xmlns:c=\"http://lca.jrc.it/ILCD/Contact\" xmlns:common=\"http://lca.jrc.it/ILCD/Common\" xmlns:epd=\"http://www.iai.kit.edu/EPD/2013\" xmlns:epd2=\"http://www.indata.network/EPD/2019\" xmlns:f=\"http://lca.jrc.it/ILCD/Flow\" xmlns:fp=\"http://lca.jrc.it/ILCD/FlowProperty\" xmlns:m=\"http://lca.jrc.it/ILCD/LCIAMethod\" xmlns:ns9=\"http://www.okworx.com/ILCD/Extensions/2018/Profile\" xmlns:s=\"http://lca.jrc.it/ILCD/Source\" xmlns:u=\"http://lca.jrc.it/ILCD/UnitGroup\" name=\"C2\"/>", "<ns11:modules xmlns:ns11=\"http://openlca.org/epd_ilcd\" xmlns=\"http://lca.jrc.it/ILCD/Process\" xmlns:c=\"http://lca.jrc.it/ILCD/Contact\" xmlns:common=\"http://lca.jrc.it/ILCD/Common\" xmlns:epd=\"http://www.iai.kit.edu/EPD/2013\" xmlns:epd2=\"http://www.indata.network/EPD/2019\" xmlns:f=\"http://lca.jrc.it/ILCD/Flow\" xmlns:fp=\"http://lca.jrc.it/ILCD/FlowProperty\" xmlns:m=\"http://lca.jrc.it/ILCD/LCIAMethod\" xmlns:ns9=\"http://www.okworx.com/ILCD/Extensions/2018/Profile\" xmlns:s=\"http://lca.jrc.it/ILCD/Source\" xmlns:u=\"http://lca.jrc.it/ILCD/UnitGroup\" name=\"C3\"/>", "<ns11:modules xmlns:ns11=\"http://openlca.org/epd_ilcd\" xmlns=\"http://lca.jrc.it/ILCD/Process\" xmlns:c=\"http://lca.jrc.it/ILCD/Contact\" xmlns:common=\"http://lca.jrc.it/ILCD/Common\" xmlns:epd=\"http://www.iai.kit.edu/EPD/2013\" xmlns:epd2=\"http://www.indata.network/EPD/2019\" xmlns:f=\"http://lca.jrc.it/ILCD/Flow\" xmlns:fp=\"http://lca.jrc.it/ILCD/FlowProperty\" xmlns:m=\"http://lca.jrc.it/ILCD/LCIAMethod\" xmlns:ns9=\"http://www.okworx.com/ILCD/Extensions/2018/Profile\" xmlns:s=\"http://lca.jrc.it/ILCD/Source\" xmlns:u=\"http://lca.jrc.it/ILCD/UnitGroup\" name=\"C4\"/>", "<ns11:modules xmlns:ns11=\"http://openlca.org/epd_ilcd\" xmlns=\"http://lca.jrc.it/ILCD/Process\" xmlns:c=\"http://lca.jrc.it/ILCD/Contact\" xmlns:common=\"http://lca.jrc.it/ILCD/Common\" xmlns:epd=\"http://www.iai.kit.edu/EPD/2013\" xmlns:epd2=\"http://www.indata.network/EPD/2019\" xmlns:f=\"http://lca.jrc.it/ILCD/Flow\" xmlns:fp=\"http://lca.jrc.it/ILCD/FlowProperty\" xmlns:m=\"http://lca.jrc.it/ILCD/LCIAMethod\" xmlns:ns9=\"http://www.okworx.com/ILCD/Extensions/2018/Profile\" xmlns:s=\"http://lca.jrc.it/ILCD/Source\" xmlns:u=\"http://lca.jrc.it/ILCD/UnitGroup\" name=\"D\"/>"]}}, "quantitativeReference": {"referenceToReferenceFlow": [1], "type": "Reference flow(s)"}, "time": {"referenceYear": 2025, "dataSetValidUntil": 2030, "timeRepresentativenessDescription": [{"value": "jährlicher Durchschnitt", "lang": "de"}, {"value": "annual average", "lang": "en"}], "other": {"anies": [{"name": "publicationDateOfEPD", "value": 1757635200000}]}}, "geography": {"locationOfOperationSupplyOrProduction": {"descriptionOfRestrictions": [{"value": "Dieser Datensatz repräsentiert die Situation des Unternehmens Roto Frank DST Produktions-GmbH , D-97980 Bad Mergentheim im Hinblick auf die wichtigsten Technologien und die gesetzlichen Rahmenbedingungen.", "lang": "de"}, {"value": "This data set represents the situation of the company Roto Frank DST Produktions-GmbH , D-97980 Bad Mergentheim with regard to the most important technologies and the legal framework.", "lang": "en"}], "location": "DE"}}, "technology": {"technologyDescriptionAndIncludedProcesses": [{"value": "Die Ökobilanzergebnisse umfassen die Lebenszyklusstadien der Herstellung der Vorprodukte bis hin zur Rohstoffgewinnung und Verarbeitungsprozesse von als Input dienenden Sekundärstoffen (z.B. Recyclingprozesse), deren Transporte zum Werk sowie die Produktion selbst, einschließlich der Bereitstellung von allen Hilfs- und Betriebsstoffen, Energie, sowie die vollständige Abfallbehandlung oder die Deponierung der Restabfälle während des Stadiums der Produktion. Die Module A1, A2 und A3 sind hier als ein aggregiertes Modul A1-A3 ausgewiesen. Falls für diesen Datensatz weitere Module berechnet wurden, sind diese separat zu finden und können für eine Betrachtung des gesamten Lebenszyklus zusammengeführt werden.", "lang": "de"}, {"value": "The life cycle assessment results cover the life cycle stages from the manufacture of primary products to the extraction of raw materials and processing of secondary materials used as input (e.g. recycling processes), their transportation to the plant and the production itself, including the provision of all auxiliary and operating materials, energy, as well as the complete waste treatment or landfilling of residual waste during the production stage. Modules A1, A2 and A3 are shown here as an aggregated module A1-A3. If further modules were calculated for this data set, these can be found separately and can be combined for a consideration of the entire life cycle.", "lang": "en"}], "technologicalApplicability": [{"value": "Plastic roof windows for installation in flat roofs with a roof pitch of 2° to 15°. The permanently integrated glazing unit efficiently provides living spaces with natural daylight and offers fall-through-proof glazing, excellent sound insulation and outstanding thermal insulation.", "lang": "en"}, {"value": "Dachflächenfenster aus Kunststoff für die Installation in Flachdächer mit einer Dachneigung von 2° bis 15°. Die fest integrierte Verglasungseinheit versorgt Wohnräume effizient mit natürlichem Tageslicht und bietet eine durchsturzsichere Verglasung, ausgezeichneten Schallschutz sowie hervorragende Wärmedämmung.", "lang": "de"}]}}, "modellingAndValidation": {"LCIMethodAndAllocation": {"typeOfDataSet": "EPD", "referenceToLCAMethodDetails": [{"shortDescription": [{"value": "Produktkategorieregeln Teil A", "lang": "de"}, {"value": "Product category rules Part A", "lang": "en"}], "type": "source data set", "refObjectId": "c6e986be-62a9-4f2f-b486-27aa9129eaeb", "version": "00.00.014"}, {"shortDescription": [{"value": "Produktkategorieregeln Teil B – für Fenster, Flachdachfenster, Lichtkuppeln und Lichtbänder", "lang": "de"}, {"value": "Product category rules Part B – for windows, flat roof windows, light domes and light bands", "lang": "en"}], "type": "source data set", "refObjectId": "8d6b7091-7bcc-4436-a2c1-98dd9aa19d6e", "version": "00.00.006"}], "other": {"anies": [{"name": "subType", "value": "specific dataset"}]}}, "dataSourcesTreatmentAndRepresentativeness": {"referenceToDataSource": [{"shortDescription": [{"value": "GaBi database (general)", "lang": "en"}], "type": "source data set", "refObjectId": "28d74cc0-db8b-4d7e-bc44-5f6d56ce0c4a", "version": "00.03.003"}], "useAdviceForDataSet": [{"value": "This data set contains the results for modules A1-A3 as well as modules A4, A5, B1, B2, B3, B4, B5, B6, B7, C1, C2, C3, C4 and D in accordance with EN 15804 + A2. \nThe modeling of the B-modules was based on 1 year.\nA comparison with other products is only permissible with a comparable application in the building. In principle, a comparison or evaluation of EPD data is only possible if all data sets to be compared were created in accordance with EN 15804 + A2 and the building context or the product-specific performance characteristics are taken into account.", "lang": "en"}, {"value": "Dieser Datensatz beinhaltet die Ergebnisse für die Module A1-A3 sowie die Module A4, A5, B1, B2, B3, B4, B5, B6, B7, C1, C2, C3, C4 und D gemäß EN 15804 + A2. Die Modellierung der B-Module wurde bezogen auf 1 Jahr vorgenommen.\r\nEin Vergleich mit anderen Produkten ist nur mit einer vergleichbaren Anwendung im Gebäude zulässig. Grundsätzlich ist eine Gegenüberstellung oder die Bewertung von EPD Daten nur möglich, wenn alle zu vergleichenden Datensätze nach EN 15804 + A2 erstellt wurden und der Gebäudekontext, bzw. die produktspezifischen Leistungsmerkmale berücksichtigt werden.", "lang": "de"}], "other": {"anies": [{"name": "referenceToOriginalEPD", "value": {"shortDescription": {"value": "EPD Flachdachfenster - Roto Frank DST - Flachdachfenster OnTop", "defaultValue": "EPD Flachdachfenster - Roto Frank DST - Flachdachfenster OnTop", "lstrings": [{"lang": "de", "value": "EPD Flachdachfenster - Roto Frank DST - Flachdachfenster OnTop"}, {"lang": "en", "value": "EPD Flat roof windows - Roto Frank DST - Flat roof windows OnTop"}]}, "version": {"version": 1, "majorVersion": 0, "minorVersion": 0, "subMinorVersion": 1, "zero": false, "versionString": "00.00.001"}, "type": "source data set", "uuid": {"uuid": "1265cead-4050-430a-9c4d-6594d8f3bc2f"}, "refObjectId": "1265cead-4050-430a-9c4d-6594d8f3bc2f", "versionAsString": "00.00.001", "resourceURLs": ["https://oekobaudat.de/OEKOBAU.DAT/resource/sources/1265cead-4050-430a-9c4d-6594d8f3bc2f/EPD-RRF-76.0.pdf?version=00.00.001", "https://oekobaudat.de/OEKOBAU.DAT/resource/sources/1265cead-4050-430a-9c4d-6594d8f3bc2f/EPD-RRF-GB-76.0.pdf?version=00.00.001"]}}]}}, "validation": {"review": [{"reviewDetails": [{"value": "Die angewendete LCI Methode ist in Übereinstimmung mit ISO 14040 und 14044. Die Dokumentation enthält alle relevanten Informationen im Hinblick auf die Datenqualität und den Umfang der Anwendung der jeweiligen LCI Ergebnisse bzw. der Datensätze. Der Datensatz repräsentiert den Stand der Technik bezogen auf die funktionelle Einheit.", "lang": "de"}, {"value": "The LCI method used is in accordance with ISO 14040 and 14044. The documentation contains all relevant information with regard to the data quality and the scope of application of the respective LCI results or data sets. The data set represents the state of the art in relation to the functional unit.", "lang": "en"}], "referenceToNameOfReviewerAndInstitution": [{"shortDescription": [{"value": "Susanne Volz", "lang": "de"}], "type": "contact data set", "refObjectId": "39da5078-3db5-40dd-bcc6-145b1dc8870d", "version": "00.00.002"}], "type": "Independent external review"}]}, "complianceDeclarations": {"compliance": [{"referenceToComplianceSystem": {"shortDescription": [{"value": "EN 15804+A2 (EF 3.1)", "lang": "de"}, {"value": "EN 15804+A2 (EF 3.1)", "lang": "en"}], "type": "source data set", "refObjectId": "d4aa3ec7-b1d7-4a4a-a6cb-37af88dcc902", "version": "00.01.000"}}]}}, "administrativeInformation": {"dataGenerator": {"referenceToPersonOrEntityGeneratingTheDataSet": [{"shortDescription": [{"value": "PeoplePlanetProfit GmbH & Co. KG", "lang": "de"}], "type": "contact data set", "refObjectId": "ca750f7c-9804-42bc-a3bd-e62bd94f4daf", "version": "00.00.001"}]}, "dataEntryBy": {"timeStamp": 1760957352599, "referenceToDataSetFormat": [{"shortDescription": [{"value": "EPD Data Format Extensions v1.2", "lang": "en"}, {"value": "EPD-Datenformaterweiterungen v1.2", "lang": "de"}], "type": "source data set", "refObjectId": "a29449fd-aa2f-4de8-b5d7-4b06b43c6fde", "version": "00.01.003"}, {"shortDescription": [{"value": "ILCD format", "lang": "en"}], "type": "source data set", "refObjectId": "a97a0155-0234-4b87-b4ce-a45da52f2a40", "version": "03.01.004", "uri": "http://lca.jrc.ec.europa.eu/lcainfohub/datasets/ilcd/sources/a97a0155-0234-4b87-b4ce-a45da52f2a40.xml"}], "referenceToPersonOrEntityEnteringTheData": {"shortDescription": [{"value": "ift Rosenheim", "lang": "de"}], "type": "contact data set", "refObjectId": "bdf65bd4-c474-4c23-8269-124ba43fa2b9", "version": "25.00.004"}}, "publicationAndOwnership": {"dataSetVersion": "00.00.008", "referenceToRegistrationAuthority": {"shortDescription": [{"value": "ift Rosenheim", "lang": "de"}], "type": "contact data set", "refObjectId": "bdf65bd4-c474-4c23-8269-124ba43fa2b9", "version": "25.00.004"}, "registrationNumber": "EPD-RFF-76.0", "referenceToOwnershipOfDataSet": {"shortDescription": [{"value": "Roto Frank DST Produktions-GmbH", "lang": "de"}], "type": "contact data set", "refObjectId": "2b614010-e115-4ca1-923c-0b677e1790ca", "version": "00.00.001"}, "copyright": true, "licenseType": "Free of charge for all users and uses", "accessRestrictions": [{"value": "none", "lang": "en"}, {"value": "keine", "lang": "de"}], "other": {"anies": [{"name": "referenceToPublisher", "value": {"shortDescription": [{"value": "ift Rosenheim", "lang": "de"}], "type": "contact data set", "refObjectId": "bdf65bd4-c474-4c23-8269-124ba43fa2b9", "version": "25.00.004"}}]}}}, "exchanges": {"exchange": [{"dataSetInternalID": 1, "referenceToFlowDataSet": {"shortDescription": [{"value": "Flachdachfenster - Roto Frank DST - Flachdachfenster OnTop Fixverglast (FF Fi)", "lang": "de"}, {"value": "flat roof window - Roto Frank DST - flat roof window OnTop Fixed glazed (FF Fi)", "lang": "en"}], "type": "flow data set", "refObjectId": "0e419984-fd52-4524-845d-bba80a38872f", "version": "00.00.004"}, "meanAmount": 1.0, "resultingAmount": 1.0, "referenceFlow": true, "resultingflowAmount": 1.0, "flowProperties": [{"name": [{"lang": "en", "value": "Carbon content (biogenic)"}], "uuid": "62e503ce-544a-4599-b2ad-bcea15a7bf20", "meanValue": 0.0}, {"name": [{"lang": "de", "value": "Fläche"}, {"lang": "en", "value": "Area"}], "uuid": "93a60a56-a3c8-19da-a746-0800200c9a66", "referenceFlowProperty": true, "meanValue": 1.0, "referenceUnit": "qm", "unitGroupUUID": "c20a03d7-bd90-4569-bc94-66cfd364dfc8"}, {"name": [{"lang": "en", "value": "Carbon content (biogenic) - packaging"}], "uuid": "262a541b-209e-44cc-a426-33bce30de7b1", "meanValue": 2.006}], "materialProperties": [{"name": "layer thickness", "value": "0.211", "unit": "m", "unitDescription": "meters"}, {"name": "grammage", "value": "54.05", "unit": "kg/m^2", "unitDescription": "kilograms per square meter"}], "typeOfFlow": "Product flow", "classification": {"classHierarchy": "Komponenten von Fenstern und Vorhangfassaden / Tageslichtsysteme und Rauch- / Wärmeabzugsanlagen  / Oberlichter", "name": "OEKOBAU.DAT"}}, {"dataSetInternalID": 2, "referenceToFlowDataSet": {"shortDescription": [{"value": "Components for re-use (CRU)", "lang": "en"}, {"value": "Komponenten für die Wiederverwendung (CRU)", "lang": "de"}, {"value": "Componentes para su reutilización (CRU)", "lang": "es"}], "type": "flow data set", "refObjectId": "a2b32f97-3fc7-4af2-b209-525bc6426f33", "version": "30.00.000", "uri": "../flows/a2b32f97-3fc7-4af2-b209-525bc6426f33.xml"}, "exchange direction": "OUTPUT", "meanAmount": 0.0, "other": {"anies": [{"value": "0.0", "module": "A1-A3"}, {"value": "0.0", "module": "A4"}, {"value": "0.0", "module": "A5"}, {"value": "0.0", "module": "B1"}, {"value": "0.0", "module": "B2"}, {"value": "0.0", "module": "B3"}, {"value": "0.0", "module": "B4"}, {"value": "0.0", "module": "B5"}, {"value": "0.0", "module": "B6"}, {"value": "0.0", "module": "B7"}, {"value": "0.0", "module": "C1"}, {"value": "0.0", "module": "C2"}, {"value": "0.0", "module": "C3"}, {"value": "0.0", "module": "C4"}, {"value": "0.0", "module": "D"}, {"name": "referenceToUnitGroupDataSet", "value": {"shortDescription": [{"value": "kg", "lang": "en"}], "type": "unit group data set", "refObjectId": "ad38d542-3fe9-439d-9b95-2f5f7752acaf", "version": "30.00.000", "uri": "../unitgroups/ad38d542-3fe9-439d-9b95-2f5f7752acaf.xml"}}]}, "flowProperties": [], "typeOfFlow": "Other flow", "classification": {"classHierarchy": "Größen / Umweltliche Größen / EPD EN 15804 / LCI Indikatoren", "name": "GaBiCategories"}}, {"dataSetInternalID": 3, "referenceToFlowDataSet": {"shortDescription": [{"value": "Exported electrical energy (EEE)", "lang": "en"}, {"value": "Exportierte elektrische Energie (EEE)", "lang": "de"}, {"value": "Energía exportada electrica (EEE)", "lang": "es"}], "type": "flow data set", "refObjectId": "4da0c987-2b76-40d6-9e9e-82a017aaaf29", "version": "30.00.000", "uri": "../flows/4da0c987-2b76-40d6-9e9e-82a017aaaf29.xml"}, "exchange direction": "OUTPUT", "meanAmount": 0.0, "other": {"anies": [{"value": "1.07", "module": "A1-A3"}, {"value": "0.0", "module": "A4"}, {"value": "15.2", "module": "A5"}, {"value": "0.0", "module": "B1"}, {"value": "0.0736", "module": "B2"}, {"value": "0.0", "module": "B3"}, {"value": "0.62", "module": "B4"}, {"value": "0.0", "module": "B5"}, {"value": "0.0", "module": "B6"}, {"value": "0.0", "module": "B7"}, {"value": "0.0", "module": "C1"}, {"value": "0.0", "module": "C2"}, {"value": "14.9", "module": "C3"}, {"value": "0.0", "module": "C4"}, {"value": "-0.14", "module": "D"}, {"name": "referenceToUnitGroupDataSet", "value": {"shortDescription": [{"value": "MJ", "lang": "en"}], "type": "unit group data set", "refObjectId": "93a60a57-a3c8-11da-a746-0800200c9a66", "version": "03.00.000", "uri": "../unitgroups/93a60a57-a3c8-11da-a746-0800200c9a66.xml"}}]}, "flowProperties": [], "typeOfFlow": "Other flow", "classification": {"classHierarchy": "Größen / Umweltliche Größen / EPD EN 15804 / LCI Indikatoren", "name": "GaBiCategories"}}, {"dataSetInternalID": 4, "referenceToFlowDataSet": {"shortDescription": [{"value": "Exported thermal energy (EET)", "lang": "en"}, {"value": "Exportierte thermische Energie (EET)", "lang": "de"}, {"value": "Energía exportada termal (EET)", "lang": "es"}], "type": "flow data set", "refObjectId": "98daf38a-7a79-46d3-9a37-2b7bd0955810", "version": "30.00.000", "uri": "../flows/98daf38a-7a79-46d3-9a37-2b7bd0955810.xml"}, "exchange direction": "OUTPUT", "meanAmount": 0.0, "other": {"anies": [{"value": "2.1", "module": "A1-A3"}, {"value": "0.0", "module": "A4"}, {"value": "30.2", "module": "A5"}, {"value": "0.0", "module": "B1"}, {"value": "0.14", "module": "B2"}, {"value": "0.0", "module": "B3"}, {"value": "1.22", "module": "B4"}, {"value": "0.0", "module": "B5"}, {"value": "0.0", "module": "B6"}, {"value": "0.0", "module": "B7"}, {"value": "0.0", "module": "C1"}, {"value": "0.0", "module": "C2"}, {"value": "28.6", "module": "C3"}, {"value": "0.0", "module": "C4"}, {"value": "-0.26", "module": "D"}, {"name": "referenceToUnitGroupDataSet", "value": {"shortDescription": [{"value": "MJ", "lang": "en"}], "type": "unit group data set", "refObjectId": "93a60a57-a3c8-11da-a746-0800200c9a66", "version": "03.00.000", "uri": "../unitgroups/93a60a57-a3c8-11da-a746-0800200c9a66.xml"}}]}, "flowProperties": [], "typeOfFlow": "Other flow", "classification": {"classHierarchy": "Größen / Umweltliche Größen / EPD EN 15804 / LCI Indikatoren", "name": "GaBiCategories"}}, {"dataSetInternalID": 5, "referenceToFlowDataSet": {"shortDescription": [{"value": "Use of net fresh water (FW)", "lang": "en"}, {"value": "Einsatz von Süßwasserressourcen (FW)", "lang": "de"}, {"value": "Uso neto de recursos de agua dulce (FW)", "lang": "es"}], "type": "flow data set", "refObjectId": "3cf952c8-f3a4-461d-8c96-96456ca62246", "version": "30.00.000", "uri": "../flows/3cf952c8-f3a4-461d-8c96-96456ca62246.xml"}, "exchange direction": "INPUT", "meanAmount": 0.0, "other": {"anies": [{"value": "0.43", "module": "A1-A3"}, {"value": "0.00398", "module": "A4"}, {"value": "0.0271", "module": "A5"}, {"value": "0.0", "module": "B1"}, {"value": "0.00308", "module": "B2"}, {"value": "0.0", "module": "B3"}, {"value": "0.008", "module": "B4"}, {"value": "0.0", "module": "B5"}, {"value": "0.0", "module": "B6"}, {"value": "0.0", "module": "B7"}, {"value": "0.0", "module": "C1"}, {"value": "8.61E-5", "module": "C2"}, {"value": "0.0353", "module": "C3"}, {"value": "0.00158", "module": "C4"}, {"value": "-0.1", "module": "D"}, {"name": "referenceToUnitGroupDataSet", "value": {"shortDescription": [{"value": "m3", "lang": "en"}], "type": "unit group data set", "refObjectId": "cd950537-0a98-4044-9ba7-9f9a68d0a504", "version": "30.00.000", "uri": "../unitgroups/cd950537-0a98-4044-9ba7-9f9a68d0a504.xml"}}]}, "flowProperties": [], "typeOfFlow": "Other flow", "classification": {"classHierarchy": "Größen / Umweltliche Größen / EPD EN 15804 / LCI Indikatoren", "name": "GaBiCategories"}}, {"dataSetInternalID": 6, "referenceToFlowDataSet": {"shortDescription": [{"value": "Hazardous waste disposed (HWD)", "lang": "en"}, {"value": "Gefährlicher Abfall zur Deponie (HWD)", "lang": "de"}, {"value": "Residuos peligrosos eliminados (HWD)", "lang": "es"}], "type": "flow data set", "refObjectId": "430f9e0f-59b2-46a0-8e0d-55e0e84948fc", "version": "30.00.000", "uri": "../flows/430f9e0f-59b2-46a0-8e0d-55e0e84948fc.xml"}, "exchange direction": "OUTPUT", "meanAmount": 0.0, "other": {"anies": [{"value": "3.28E-6", "module": "A1-A3"}, {"value": "4.28E-9", "module": "A4"}, {"value": "1.52E-9", "module": "A5"}, {"value": "0.0", "module": "B1"}, {"value": "4.3E-8", "module": "B2"}, {"value": "0.0", "module": "B3"}, {"value": "6.4E-8", "module": "B4"}, {"value": "0.0", "module": "B5"}, {"value": "0.0", "module": "B6"}, {"value": "0.0", "module": "B7"}, {"value": "0.0", "module": "C1"}, {"value": "9.27E-11", "module": "C2"}, {"value": "3.1E-8", "module": "C3"}, {"value": "1.43E-9", "module": "C4"}, {"value": "-1.36E-6", "module": "D"}, {"name": "referenceToUnitGroupDataSet", "value": {"shortDescription": [{"value": "kg", "lang": "en"}], "type": "unit group data set", "refObjectId": "ad38d542-3fe9-439d-9b95-2f5f7752acaf", "version": "30.00.000", "uri": "../unitgroups/ad38d542-3fe9-439d-9b95-2f5f7752acaf.xml"}}]}, "flowProperties": [], "typeOfFlow": "Other flow", "classification": {"classHierarchy": "Größen / Umweltliche Größen / EPD EN 15804 / LCI Indikatoren", "name": "GaBiCategories"}}, {"dataSetInternalID": 7, "referenceToFlowDataSet": {"shortDescription": [{"value": "Materials for energy recovery (MER)", "lang": "en"}, {"value": "Stoffe für die Energierückgewinnung (MER)", "lang": "de"}, {"value": "Materiales para valorización energética (recuperación de energía) (MER)", "lang": "es"}], "type": "flow data set", "refObjectId": "59a9181c-3aaf-46ee-8b13-2b3723b6e447", "version": "30.00.000", "uri": "../flows/59a9181c-3aaf-46ee-8b13-2b3723b6e447.xml"}, "exchange direction": "OUTPUT", "meanAmount": 0.0, "other": {"anies": [{"value": "0.0", "module": "A1-A3"}, {"value": "0.0", "module": "A4"}, {"value": "0.0", "module": "A5"}, {"value": "0.0", "module": "B1"}, {"value": "0.0", "module": "B2"}, {"value": "0.0", "module": "B3"}, {"value": "0.0", "module": "B4"}, {"value": "0.0", "module": "B5"}, {"value": "0.0", "module": "B6"}, {"value": "0.0", "module": "B7"}, {"value": "0.0", "module": "C1"}, {"value": "0.0", "module": "C2"}, {"value": "0.0", "module": "C3"}, {"value": "0.0", "module": "C4"}, {"value": "0.0", "module": "D"}, {"name": "referenceToUnitGroupDataSet", "value": {"shortDescription": [{"value": "kg", "lang": "en"}], "type": "unit group data set", "refObjectId": "ad38d542-3fe9-439d-9b95-2f5f7752acaf", "version": "30.00.000", "uri": "../unitgroups/ad38d542-3fe9-439d-9b95-2f5f7752acaf.xml"}}]}, "flowProperties": [], "typeOfFlow": "Other flow", "classification": {"classHierarchy": "Größen / Umweltliche Größen / EPD EN 15804 / LCI Indikatoren", "name": "GaBiCategories"}}, {"dataSetInternalID": 8, "referenceToFlowDataSet": {"shortDescription": [{"value": "Materials for recycling (MFR)", "lang": "en"}, {"value": "Stoffe zum Recycling (MFR)", "lang": "de"}, {"value": "Materiales para el reciclaje (MFR)", "lang": "es"}], "type": "flow data set", "refObjectId": "d7fe48a5-4103-49c8-9aae-b0b5dfdbd6ae", "version": "30.00.000", "uri": "../flows/d7fe48a5-4103-49c8-9aae-b0b5dfdbd6ae.xml"}, "exchange direction": "OUTPUT", "meanAmount": 0.0, "other": {"anies": [{"value": "6.16", "module": "A1-A3"}, {"value": "0.0", "module": "A4"}, {"value": "0.0", "module": "A5"}, {"value": "0.0", "module": "B1"}, {"value": "0.87", "module": "B2"}, {"value": "0.0", "module": "B3"}, {"value": "0.45", "module": "B4"}, {"value": "0.0", "module": "B5"}, {"value": "0.0", "module": "B6"}, {"value": "0.0", "module": "B7"}, {"value": "0.0", "module": "C1"}, {"value": "0.0", "module": "C2"}, {"value": "16.4", "module": "C3"}, {"value": "0.0", "module": "C4"}, {"value": "-0.00608", "module": "D"}, {"name": "referenceToUnitGroupDataSet", "value": {"shortDescription": [{"value": "kg", "lang": "en"}], "type": "unit group data set", "refObjectId": "ad38d542-3fe9-439d-9b95-2f5f7752acaf", "version": "30.00.000", "uri": "../unitgroups/ad38d542-3fe9-439d-9b95-2f5f7752acaf.xml"}}]}, "flowProperties": [], "typeOfFlow": "Other flow", "classification": {"classHierarchy": "Größen / Umweltliche Größen / EPD EN 15804 / LCI Indikatoren", "name": "GaBiCategories"}}, {"dataSetInternalID": 9, "referenceToFlowDataSet": {"shortDescription": [{"value": "Non-hazardous waste disposed (NHWD)", "lang": "en"}, {"value": "Entsorgter nicht gefährlicher Abfall (NHWD)", "lang": "de"}, {"value": "Residuos no peligrosos eliminados (NHWD)", "lang": "es"}], "type": "flow data set", "refObjectId": "b29ef66b-e286-4afa-949f-62f1a7b4d7fa", "version": "30.00.000", "uri": "../flows/b29ef66b-e286-4afa-949f-62f1a7b4d7fa.xml"}, "exchange direction": "OUTPUT", "meanAmount": 0.0, "other": {"anies": [{"value": "11.69", "module": "A1-A3"}, {"value": "0.0149", "module": "A4"}, {"value": "0.19", "module": "A5"}, {"value": "0.0", "module": "B1"}, {"value": "0.0646", "module": "B2"}, {"value": "0.0", "module": "B3"}, {"value": "0.91", "module": "B4"}, {"value": "0.0", "module": "B5"}, {"value": "0.0", "module": "B6"}, {"value": "0.0", "module": "B7"}, {"value": "0.0", "module": "C1"}, {"value": "3.23E-4", "module": "C2"}, {"value": "3.16", "module": "C3"}, {"value": "32.7", "module": "C4"}, {"value": "-3.68", "module": "D"}, {"name": "referenceToUnitGroupDataSet", "value": {"shortDescription": [{"value": "kg", "lang": "en"}], "type": "unit group data set", "refObjectId": "ad38d542-3fe9-439d-9b95-2f5f7752acaf", "version": "30.00.000", "uri": "../unitgroups/ad38d542-3fe9-439d-9b95-2f5f7752acaf.xml"}}]}, "flowProperties": [], "typeOfFlow": "Other flow", "classification": {"classHierarchy": "Größen / Umweltliche Größen / EPD EN 15804 / LCI Indikatoren", "name": "GaBiCategories"}}, {"dataSetInternalID": 10, "referenceToFlowDataSet": {"shortDescription": [{"value": "Use of non renewable secondary fuels (NRSF)", "lang": "en"}, {"value": "Nicht erneuerbare Sekundärbrennstoffe (NRSF)", "lang": "de"}, {"value": "Uso de combustibles secundarios no renovables (NRSF)", "lang": "es"}], "type": "flow data set", "refObjectId": "89def144-d39a-4287-b86f-efde453ddcb2", "version": "30.00.000", "uri": "../flows/89def144-d39a-4287-b86f-efde453ddcb2.xml"}, "exchange direction": "INPUT", "meanAmount": 0.0, "other": {"anies": [{"value": "0.0", "module": "A1-A3"}, {"value": "0.0", "module": "A4"}, {"value": "0.0", "module": "A5"}, {"value": "0.0", "module": "B1"}, {"value": "0.0", "module": "B2"}, {"value": "0.0", "module": "B3"}, {"value": "0.0", "module": "B4"}, {"value": "0.0", "module": "B5"}, {"value": "0.0", "module": "B6"}, {"value": "0.0", "module": "B7"}, {"value": "0.0", "module": "C1"}, {"value": "0.0", "module": "C2"}, {"value": "0.0", "module": "C3"}, {"value": "0.0", "module": "C4"}, {"value": "0.0", "module": "D"}, {"name": "referenceToUnitGroupDataSet", "value": {"shortDescription": [{"value": "MJ", "lang": "en"}], "type": "unit group data set", "refObjectId": "93a60a57-a3c8-11da-a746-0800200c9a66", "version": "03.00.000", "uri": "../unitgroups/93a60a57-a3c8-11da-a746-0800200c9a66.xml"}}]}, "flowProperties": [], "typeOfFlow": "Other flow", "classification": {"classHierarchy": "Größen / Umweltliche Größen / EPD EN 15804 / LCI Indikatoren", "name": "GaBiCategories"}}, {"dataSetInternalID": 11, "referenceToFlowDataSet": {"shortDescription": [{"value": "Use of non renewable primary energy (PENRE)", "lang": "en"}, {"value": "Nicht-erneuerbare Primärenergie als Energieträger (PENRE)", "lang": "de"}, {"value": "Uso de energía primaria no renovable, excluyendo los recursos de energía primaria no renovable utilizada como materia prima (PENRE)", "lang": "es"}], "type": "flow data set", "refObjectId": "ac857178-2b45-46ec-892a-a9a4332f0372", "version": "38.00.000", "uri": "../flows/ac857178-2b45-46ec-892a-a9a4332f0372.xml"}, "exchange direction": "INPUT", "meanAmount": 0.0, "other": {"anies": [{"value": "1736.0", "module": "A1-A3"}, {"value": "107.0", "module": "A4"}, {"value": "25.07", "module": "A5"}, {"value": "0.0", "module": "B1"}, {"value": "14.68", "module": "B2"}, {"value": "0.0", "module": "B3"}, {"value": "35.43", "module": "B4"}, {"value": "0.0", "module": "B5"}, {"value": "0.0", "module": "B6"}, {"value": "0.0", "module": "B7"}, {"value": "0.0", "module": "C1"}, {"value": "2.31", "module": "C2"}, {"value": "137.4", "module": "C3"}, {"value": "6.55", "module": "C4"}, {"value": "-634.0", "module": "D"}, {"name": "referenceToUnitGroupDataSet", "value": {"shortDescription": [{"value": "MJ", "lang": "en"}], "type": "unit group data set", "refObjectId": "93a60a57-a3c8-11da-a746-0800200c9a66", "version": "03.00.000", "uri": "../unitgroups/93a60a57-a3c8-11da-a746-0800200c9a66.xml"}}]}, "flowProperties": [], "typeOfFlow": "Other flow", "classification": {"classHierarchy": "Quantities", "name": "GaBiCategories"}}, {"dataSetInternalID": 12, "referenceToFlowDataSet": {"shortDescription": [{"value": "Use of non renewable primary energy resources used as raw materials (PENRM)", "lang": "en"}, {"value": "Nicht-erneuerbare Primärenergie zur stofflichen Nutzung (PENRM)", "lang": "de"}, {"value": "Uso de la energía primaria no renovable utilizada como materia prima (PENRM)", "lang": "es"}], "type": "flow data set", "refObjectId": "1421caa0-679d-4bf4-b282-0eb850ccae27", "version": "38.00.000", "uri": "../flows/1421caa0-679d-4bf4-b282-0eb850ccae27.xml"}, "exchange direction": "INPUT", "meanAmount": 0.0, "other": {"anies": [{"value": "164.0", "module": "A1-A3"}, {"value": "0.0", "module": "A4"}, {"value": "-22.4", "module": "A5"}, {"value": "0.0", "module": "B1"}, {"value": "0.0", "module": "B2"}, {"value": "0.0", "module": "B3"}, {"value": "0.71", "module": "B4"}, {"value": "0.0", "module": "B5"}, {"value": "0.0", "module": "B6"}, {"value": "0.0", "module": "B7"}, {"value": "0.0", "module": "C1"}, {"value": "0.0", "module": "C2"}, {"value": "-106.0", "module": "C3"}, {"value": "0.0", "module": "C4"}, {"value": "0.0", "module": "D"}, {"name": "referenceToUnitGroupDataSet", "value": {"shortDescription": [{"value": "MJ", "lang": "en"}], "type": "unit group data set", "refObjectId": "93a60a57-a3c8-11da-a746-0800200c9a66", "version": "03.00.000", "uri": "../unitgroups/93a60a57-a3c8-11da-a746-0800200c9a66.xml"}}]}, "flowProperties": [], "typeOfFlow": "Other flow", "classification": {"classHierarchy": "Quantities", "name": "GaBiCategories"}}, {"dataSetInternalID": 13, "referenceToFlowDataSet": {"shortDescription": [{"value": "Total use of non-renewable primary energy resources (PENRT)", "lang": "en"}, {"value": "Total nicht erneuerbare Primärenergie (PENRT)", "lang": "de"}, {"value": "Uso total de la energía primaria no renovable (energía primaria y recursos de energía primaria renovable utilizada como materia prima) (PENRT)", "lang": "es"}], "type": "flow data set", "refObjectId": "06159210-646b-4c8d-8583-da9b3b95a6c1", "version": "30.00.000", "uri": "../flows/06159210-646b-4c8d-8583-da9b3b95a6c1.xml"}, "exchange direction": "INPUT", "meanAmount": 0.0, "other": {"anies": [{"value": "1900.0", "module": "A1-A3"}, {"value": "107.0", "module": "A4"}, {"value": "2.67", "module": "A5"}, {"value": "0.0", "module": "B1"}, {"value": "14.68", "module": "B2"}, {"value": "0.0", "module": "B3"}, {"value": "36.14", "module": "B4"}, {"value": "0.0", "module": "B5"}, {"value": "0.0", "module": "B6"}, {"value": "0.0", "module": "B7"}, {"value": "0.0", "module": "C1"}, {"value": "2.31", "module": "C2"}, {"value": "31.4", "module": "C3"}, {"value": "6.55", "module": "C4"}, {"value": "-634.0", "module": "D"}, {"name": "referenceToUnitGroupDataSet", "value": {"shortDescription": [{"value": "MJ", "lang": "en"}], "type": "unit group data set", "refObjectId": "93a60a57-a3c8-11da-a746-0800200c9a66", "version": "03.00.000", "uri": "../unitgroups/93a60a57-a3c8-11da-a746-0800200c9a66.xml"}}]}, "flowProperties": [], "typeOfFlow": "Other flow", "classification": {"classHierarchy": "Größen / Umweltliche Größen / EPD EN 15804 / LCI Indikatoren", "name": "GaBiCategories"}}, {"dataSetInternalID": 14, "referenceToFlowDataSet": {"shortDescription": [{"value": "Use of renewable primary energy (PERE)", "lang": "en"}, {"value": "Erneuerbare Primärenergie als Energieträger (PERE)", "lang": "de"}, {"value": "Uso de energía primaria renovable excluyendo los recursos de energía primaria renovable utilizada como materia prima (PERE)", "lang": "es"}], "type": "flow data set", "refObjectId": "20f32be5-0398-4288-9b6d-accddd195317", "version": "38.00.000", "uri": "../flows/20f32be5-0398-4288-9b6d-accddd195317.xml"}, "exchange direction": "INPUT", "meanAmount": 0.0, "other": {"anies": [{"value": "528.9", "module": "A1-A3"}, {"value": "8.05", "module": "A4"}, {"value": "92.5", "module": "A5"}, {"value": "0.0", "module": "B1"}, {"value": "1.6", "module": "B2"}, {"value": "0.0", "module": "B3"}, {"value": "11.38", "module": "B4"}, {"value": "0.0", "module": "B5"}, {"value": "0.0", "module": "B6"}, {"value": "0.0", "module": "B7"}, {"value": "0.0", "module": "C1"}, {"value": "0.17", "module": "C2"}, {"value": "16.31", "module": "C3"}, {"value": "1.26", "module": "C4"}, {"value": "-107.4", "module": "D"}, {"name": "referenceToUnitGroupDataSet", "value": {"shortDescription": [{"value": "MJ", "lang": "en"}], "type": "unit group data set", "refObjectId": "93a60a57-a3c8-11da-a746-0800200c9a66", "version": "03.00.000", "uri": "../unitgroups/93a60a57-a3c8-11da-a746-0800200c9a66.xml"}}]}, "flowProperties": [], "typeOfFlow": "Other flow", "classification": {"classHierarchy": "Quantities", "name": "GaBiCategories"}}, {"dataSetInternalID": 15, "referenceToFlowDataSet": {"shortDescription": [{"value": "Use of renewable primary energy resources used as raw materials (PERM)", "lang": "en"}, {"value": "Erneuerbare Primärenergie zur stofflichen Nutzung (PERM)", "lang": "de"}, {"value": "Uso de energía primaria renovable utilizada como materia prima (PERM)", "lang": "es"}], "type": "flow data set", "refObjectId": "fb3ec0de-548d-4508-aea5-00b73bf6f702", "version": "38.00.000", "uri": "../flows/fb3ec0de-548d-4508-aea5-00b73bf6f702.xml"}, "exchange direction": "INPUT", "meanAmount": 0.0, "other": {"anies": [{"value": "92.2", "module": "A1-A3"}, {"value": "0.0", "module": "A4"}, {"value": "-91.77", "module": "A5"}, {"value": "0.0", "module": "B1"}, {"value": "0.0", "module": "B2"}, {"value": "0.0", "module": "B3"}, {"value": "0.00251", "module": "B4"}, {"value": "0.0", "module": "B5"}, {"value": "0.0", "module": "B6"}, {"value": "0.0", "module": "B7"}, {"value": "0.0", "module": "C1"}, {"value": "0.0", "module": "C2"}, {"value": "-0.31", "module": "C3"}, {"value": "0.0", "module": "C4"}, {"value": "0.0", "module": "D"}, {"name": "referenceToUnitGroupDataSet", "value": {"shortDescription": [{"value": "MJ", "lang": "en"}], "type": "unit group data set", "refObjectId": "93a60a57-a3c8-11da-a746-0800200c9a66", "version": "03.00.000", "uri": "../unitgroups/93a60a57-a3c8-11da-a746-0800200c9a66.xml"}}]}, "flowProperties": [], "typeOfFlow": "Other flow", "classification": {"classHierarchy": "Quantities", "name": "GaBiCategories"}}, {"dataSetInternalID": 16, "referenceToFlowDataSet": {"shortDescription": [{"value": "Total use of renewable primary energy resources (PERT)", "lang": "en"}, {"value": "Total erneuerbare Primärenergie (PERT)", "lang": "de"}, {"value": "Uso total de la energía primaria renovable (energía primaria y recursos de energía primaria renovable utilizada como materia prima) (PERT)", "lang": "es"}], "type": "flow data set", "refObjectId": "53f97275-fa8a-4cdd-9024-65936002acd0", "version": "30.00.000", "uri": "../flows/53f97275-fa8a-4cdd-9024-65936002acd0.xml"}, "exchange direction": "INPUT", "meanAmount": 0.0, "other": {"anies": [{"value": "621.1", "module": "A1-A3"}, {"value": "8.05", "module": "A4"}, {"value": "0.73", "module": "A5"}, {"value": "0.0", "module": "B1"}, {"value": "1.6", "module": "B2"}, {"value": "0.0", "module": "B3"}, {"value": "11.38", "module": "B4"}, {"value": "0.0", "module": "B5"}, {"value": "0.0", "module": "B6"}, {"value": "0.0", "module": "B7"}, {"value": "0.0", "module": "C1"}, {"value": "0.17", "module": "C2"}, {"value": "16.0", "module": "C3"}, {"value": "1.26", "module": "C4"}, {"value": "-107.4", "module": "D"}, {"name": "referenceToUnitGroupDataSet", "value": {"shortDescription": [{"value": "MJ", "lang": "en"}], "type": "unit group data set", "refObjectId": "93a60a57-a3c8-11da-a746-0800200c9a66", "version": "03.00.000", "uri": "../unitgroups/93a60a57-a3c8-11da-a746-0800200c9a66.xml"}}]}, "flowProperties": [], "typeOfFlow": "Other flow", "classification": {"classHierarchy": "Größen / Umweltliche Größen / EPD EN 15804 / LCI Indikatoren", "name": "GaBiCategories"}}, {"dataSetInternalID": 17, "referenceToFlowDataSet": {"shortDescription": [{"value": "Use of renewable secondary fuels (RSF)", "lang": "en"}, {"value": "Erneuerbare Sekundärbrennstoffe (RSF)", "lang": "de"}, {"value": "Uso de combustibles secundarios renovables (RSF)", "lang": "es"}], "type": "flow data set", "refObjectId": "64333088-a55f-4aa2-9a31-c10b07816787", "version": "30.00.000", "uri": "../flows/64333088-a55f-4aa2-9a31-c10b07816787.xml"}, "exchange direction": "INPUT", "meanAmount": 0.0, "other": {"anies": [{"value": "0.0", "module": "A1-A3"}, {"value": "0.0", "module": "A4"}, {"value": "0.0", "module": "A5"}, {"value": "0.0", "module": "B1"}, {"value": "0.0", "module": "B2"}, {"value": "0.0", "module": "B3"}, {"value": "0.0", "module": "B4"}, {"value": "0.0", "module": "B5"}, {"value": "0.0", "module": "B6"}, {"value": "0.0", "module": "B7"}, {"value": "0.0", "module": "C1"}, {"value": "0.0", "module": "C2"}, {"value": "0.0", "module": "C3"}, {"value": "0.0", "module": "C4"}, {"value": "0.0", "module": "D"}, {"name": "referenceToUnitGroupDataSet", "value": {"shortDescription": [{"value": "MJ", "lang": "en"}], "type": "unit group data set", "refObjectId": "93a60a57-a3c8-11da-a746-0800200c9a66", "version": "03.00.000", "uri": "../unitgroups/93a60a57-a3c8-11da-a746-0800200c9a66.xml"}}]}, "flowProperties": [], "typeOfFlow": "Other flow", "classification": {"classHierarchy": "Größen / Umweltliche Größen / EPD EN 15804 / LCI Indikatoren", "name": "GaBiCategories"}}, {"dataSetInternalID": 18, "referenceToFlowDataSet": {"shortDescription": [{"value": "Radioactive waste disposed (RWD)", "lang": "en"}, {"value": "Entsorgter radioaktiver Abfall (RWD)", "lang": "de"}, {"value": "Residuos radiactivos eliminados (RWD)", "lang": "es"}], "type": "flow data set", "refObjectId": "3449546e-52ad-4b39-b809-9fb77cea8ff6", "version": "30.00.000", "uri": "../flows/3449546e-52ad-4b39-b809-9fb77cea8ff6.xml"}, "exchange direction": "OUTPUT", "meanAmount": 0.0, "other": {"anies": [{"value": "0.029", "module": "A1-A3"}, {"value": "2.02E-4", "module": "A4"}, {"value": "1.16E-4", "module": "A5"}, {"value": "0.0", "module": "B1"}, {"value": "4.3E-8", "module": "B2"}, {"value": "0.0", "module": "B3"}, {"value": "6.4E-8", "module": "B4"}, {"value": "0.0", "module": "B5"}, {"value": "0.0", "module": "B6"}, {"value": "0.0", "module": "B7"}, {"value": "0.0", "module": "C1"}, {"value": "4.36E-6", "module": "C2"}, {"value": "0.00334", "module": "C3"}, {"value": "6.94E-5", "module": "C4"}, {"value": "-0.0177", "module": "D"}, {"name": "referenceToUnitGroupDataSet", "value": {"shortDescription": [{"value": "kg", "lang": "en"}], "type": "unit group data set", "refObjectId": "ad38d542-3fe9-439d-9b95-2f5f7752acaf", "version": "30.00.000", "uri": "../unitgroups/ad38d542-3fe9-439d-9b95-2f5f7752acaf.xml"}}]}, "flowProperties": [], "typeOfFlow": "Other flow", "classification": {"classHierarchy": "Größen / Umweltliche Größen / EPD EN 15804 / LCI Indikatoren", "name": "GaBiCategories"}}, {"dataSetInternalID": 19, "referenceToFlowDataSet": {"shortDescription": [{"value": "Use of secondary material (SM)", "lang": "en"}, {"value": "Einsatz von Sekundärstoffen (SM)", "lang": "de"}, {"value": "Uso de materiales secundarios (SM)", "lang": "es"}], "type": "flow data set", "refObjectId": "c6a1f35f-2d09-4f54-8dfb-97e502e1ce92", "version": "30.00.000", "uri": "../flows/c6a1f35f-2d09-4f54-8dfb-97e502e1ce92.xml"}, "exchange direction": "INPUT", "meanAmount": 0.0, "other": {"anies": [{"value": "9.45", "module": "A1-A3"}, {"value": "0.0", "module": "A4"}, {"value": "0.0", "module": "A5"}, {"value": "0.0", "module": "B1"}, {"value": "0.19", "module": "B2"}, {"value": "0.0", "module": "B3"}, {"value": "0.19", "module": "B4"}, {"value": "0.0", "module": "B5"}, {"value": "0.0", "module": "B6"}, {"value": "0.0", "module": "B7"}, {"value": "0.0", "module": "C1"}, {"value": "0.0", "module": "C2"}, {"value": "0.0", "module": "C3"}, {"value": "0.0", "module": "C4"}, {"value": "-5.62", "module": "D"}, {"name": "referenceToUnitGroupDataSet", "value": {"shortDescription": [{"value": "kg", "lang": "en"}], "type": "unit group data set", "refObjectId": "ad38d542-3fe9-439d-9b95-2f5f7752acaf", "version": "30.00.000", "uri": "../unitgroups/ad38d542-3fe9-439d-9b95-2f5f7752acaf.xml"}}]}, "flowProperties": [], "typeOfFlow": "Other flow", "classification": {"classHierarchy": "Größen / Umweltliche Größen / EPD EN 15804 / LCI Indikatoren", "name": "GaBiCategories"}}]}, "LCIAResults": {"LCIAResult": [{"referenceToLCIAMethodDataSet": {"shortDescription": [{"value": "Abiotic depletion potential - non-fossil resources (ADPE)", "lang": "en"}, {"value": "Potenzial für die Verknappung abiotischer Ressourcen – nicht fossile Ressourcen (ADPE)", "lang": "de"}], "type": "LCIA method data set", "refObjectId": "b2ad6494-c78d-11e6-9d9d-cec0c932ce01", "version": "01.00.011", "uri": "../lciamethods/b2ad6494-c78d-11e6-9d9d-cec0c932ce01.xml"}, "meanAmount": 0.0, "other": {"anies": [{"value": "1.73E-4", "module": "A1-A3"}, {"value": "5.54E-7", "module": "A4"}, {"value": "1.51E-8", "module": "A5"}, {"value": "0.0", "module": "B1"}, {"value": "7.68E-7", "module": "B2"}, {"value": "0.0", "module": "B3"}, {"value": "3.42E-6", "module": "B4"}, {"value": "0.0", "module": "B5"}, {"value": "0.0", "module": "B6"}, {"value": "0.0", "module": "B7"}, {"value": "0.0", "module": "C1"}, {"value": "1.2E-8", "module": "C2"}, {"value": "2.6E-7", "module": "C3"}, {"value": "3.09E-8", "module": "C4"}, {"value": "-3.32E-6", "module": "D"}, {"name": "referenceToUnitGroupDataSet", "value": {"shortDescription": [{"value": "kg Sb-eq.", "lang": "en"}], "type": "unit group data set", "refObjectId": "54ccd2d9-a32a-4fc2-923d-f2c8c93e89d4", "version": "30.00.000", "uri": "../unitgroups/54ccd2d9-a32a-4fc2-923d-f2c8c93e89d4.xml"}}]}}, {"referenceToLCIAMethodDataSet": {"shortDescription": [{"value": "Abiotic depletion potential - fossil resources (ADPF)", "lang": "en"}, {"value": "Potenzial für die Verknappung abiotischer Ressourcen – fossile Brennstoffe (ADPF)", "lang": "de"}], "type": "LCIA method data set", "refObjectId": "b2ad6110-c78d-11e6-9d9d-cec0c932ce01", "version": "01.00.011", "uri": "../lciamethods/b2ad6110-c78d-11e6-9d9d-cec0c932ce01.xml"}, "meanAmount": 0.0, "other": {"anies": [{"value": "1900.0", "module": "A1-A3"}, {"value": "107.0", "module": "A4"}, {"value": "2.67", "module": "A5"}, {"value": "0.0", "module": "B1"}, {"value": "14.74", "module": "B2"}, {"value": "0.0", "module": "B3"}, {"value": "36.14", "module": "B4"}, {"value": "0.0", "module": "B5"}, {"value": "0.0", "module": "B6"}, {"value": "0.0", "module": "B7"}, {"value": "0.0", "module": "C1"}, {"value": "2.31", "module": "C2"}, {"value": "31.4", "module": "C3"}, {"value": "6.55", "module": "C4"}, {"value": "-634.0", "module": "D"}, {"name": "referenceToUnitGroupDataSet", "value": {"shortDescription": [{"value": "MJ", "lang": "en"}], "type": "unit group data set", "refObjectId": "93a60a57-a3c8-11da-a746-0800200c9a66", "version": "03.00.000", "uri": "../unitgroups/93a60a57-a3c8-11da-a746-0800200c9a66.xml"}}]}}, {"referenceToLCIAMethodDataSet": {"shortDescription": [{"value": "Acidification potential, Accumulated Exceedance (AP)", "lang": "en"}, {"value": "Versauerungspotenzial, kumulierte Überschreitung (AP)", "lang": "de"}], "type": "LCIA method data set", "refObjectId": "b5c611c6-def3-11e6-bf01-fe55135034f3", "version": "01.03.010", "uri": "../lciamethods/b5c611c6-def3-11e6-bf01-fe55135034f3.xml"}, "meanAmount": 0.0, "other": {"anies": [{"value": "0.42", "module": "A1-A3"}, {"value": "0.0197", "module": "A4"}, {"value": "0.00225", "module": "A5"}, {"value": "0.0", "module": "B1"}, {"value": "0.00432", "module": "B2"}, {"value": "0.0", "module": "B3"}, {"value": "0.00822", "module": "B4"}, {"value": "0.0", "module": "B5"}, {"value": "0.0", "module": "B6"}, {"value": "0.0", "module": "B7"}, {"value": "0.0", "module": "C1"}, {"value": "2.49E-4", "module": "C2"}, {"value": "0.00447", "module": "C3"}, {"value": "0.00353", "module": "C4"}, {"value": "-0.15", "module": "D"}, {"name": "referenceToUnitGroupDataSet", "value": {"shortDescription": [{"value": "mol H+-eq.", "lang": "en"}], "type": "unit group data set", "refObjectId": "42e089ac-92bf-4bf2-8ca1-5fc40d18f2ed", "version": "00.01.000", "uri": "../unitgroups/42e089ac-92bf-4bf2-8ca1-5fc40d18f2ed.xml"}}]}}, {"referenceToLCIAMethodDataSet": {"shortDescription": [{"value": "Eutrophication potential - freshwater (EP-freshwater)", "lang": "en"}, {"value": "Eutrophierungspotenzial - Süßwasser (EP-freshwater)", "lang": "de"}], "type": "LCIA method data set", "refObjectId": "b53ec18f-7377-4ad3-86eb-cc3f4f276b2b", "version": "01.00.011", "uri": "../lciamethods/b53ec18f-7377-4ad3-86eb-cc3f4f276b2b.xml"}, "meanAmount": 0.0, "other": {"anies": [{"value": "2650.0", "module": "A1-A3"}, {"value": "2.25E-5", "module": "A4"}, {"value": "2.23E-7", "module": "A5"}, {"value": "0.0", "module": "B1"}, {"value": "53.0", "module": "B2"}, {"value": "0.0", "module": "B3"}, {"value": "53.0", "module": "B4"}, {"value": "0.0", "module": "B5"}, {"value": "0.0", "module": "B6"}, {"value": "0.0", "module": "B7"}, {"value": "0.0", "module": "C1"}, {"value": "4.86E-7", "module": "C2"}, {"value": "3.01E-6", "module": "C3"}, {"value": "7.43E-7", "module": "C4"}, {"value": "-1550.0", "module": "D"}, {"name": "referenceToUnitGroupDataSet", "value": {"shortDescription": [{"value": "kg P-eq.", "lang": "en"}], "type": "unit group data set", "refObjectId": "0429039d-a61d-4590-ba67-aa4a20a810a1", "version": "30.00.000", "uri": "../unitgroups/0429039d-a61d-4590-ba67-aa4a20a810a1.xml"}}]}}, {"referenceToLCIAMethodDataSet": {"shortDescription": [{"value": "Eutrophication potential - marine (EP-marine)", "lang": "en"}, {"value": "Eutrophierungspotenzial - Salzwasser (EP-marine)", "lang": "de"}], "type": "LCIA method data set", "refObjectId": "b5c619fa-def3-11e6-bf01-fe55135034f3", "version": "02.00.011", "uri": "../lciamethods/b5c619fa-def3-11e6-bf01-fe55135034f3.xml"}, "meanAmount": 0.0, "other": {"anies": [{"value": "0.0949", "module": "A1-A3"}, {"value": "0.00879", "module": "A4"}, {"value": "7.39E-4", "module": "A5"}, {"value": "0.0", "module": "B1"}, {"value": "8.76E-4", "module": "B2"}, {"value": "0.0", "module": "B3"}, {"value": "0.00195", "module": "B4"}, {"value": "0.0", "module": "B5"}, {"value": "0.0", "module": "B6"}, {"value": "0.0", "module": "B7"}, {"value": "0.0", "module": "C1"}, {"value": "1.0E-4", "module": "C2"}, {"value": "0.00127", "module": "C3"}, {"value": "9.23E-4", "module": "C4"}, {"value": "-0.0333", "module": "D"}, {"name": "referenceToUnitGroupDataSet", "value": {"shortDescription": [{"value": "kg N-eq.", "lang": "en"}], "type": "unit group data set", "refObjectId": "d05bb823-ecdf-4686-8c40-bf1d9257859f", "version": "00.00.003", "uri": "../unitgroups/d05bb823-ecdf-4686-8c40-bf1d9257859f.xml"}}]}}, {"referenceToLCIAMethodDataSet": {"shortDescription": [{"value": "Eutrophication potential - terrestrial (EP-terrestrial)", "lang": "en"}, {"value": "Eutrophierungspotenzial - Land (EP-terrestrial)", "lang": "de"}], "type": "LCIA method data set", "refObjectId": "b5c614d2-def3-11e6-bf01-fe55135034f3", "version": "01.02.010", "uri": "../lciamethods/b5c614d2-def3-11e6-bf01-fe55135034f3.xml"}, "meanAmount": 0.0, "other": {"anies": [{"value": "1.17", "module": "A1-A3"}, {"value": "0.0947", "module": "A4"}, {"value": "0.0105", "module": "A5"}, {"value": "0.0", "module": "B1"}, {"value": "0.0125", "module": "B2"}, {"value": "0.0", "module": "B3"}, {"value": "0.0241", "module": "B4"}, {"value": "0.0", "module": "B5"}, {"value": "0.0", "module": "B6"}, {"value": "0.0", "module": "B7"}, {"value": "0.0", "module": "C1"}, {"value": "0.00104", "module": "C2"}, {"value": "0.0162", "module": "C3"}, {"value": "0.0101", "module": "C4"}, {"value": "-0.45", "module": "D"}, {"name": "referenceToUnitGroupDataSet", "value": {"shortDescription": [{"value": "mol N-eq.", "lang": "en"}], "type": "unit group data set", "refObjectId": "71b4d617-0ec9-4d3f-b65e-e438940c2401", "version": "00.00.003", "uri": "../unitgroups/71b4d617-0ec9-4d3f-b65e-e438940c2401.xml"}}]}}, {"referenceToLCIAMethodDataSet": {"shortDescription": [{"value": "Potential Comparative Toxic Unit for ecosystems (ETP-fw)", "lang": "en"}, {"value": "Potenzielle Toxizitätsvergleichseinheit für Ökosysteme (ETP-fw)", "lang": "de"}], "type": "LCIA method data set", "refObjectId": "05316e7a-b254-4bea-9cf0-6bf33eb5c630", "version": "01.00.003", "uri": "../lciamethods/05316e7a-b254-4bea-9cf0-6bf33eb5c630.xml"}, "meanAmount": 0.0, "other": {"anies": [{"value": "753.0", "module": "A1-A3"}, {"value": "139.0", "module": "A4"}, {"value": "1.06", "module": "A5"}, {"value": "0.0", "module": "B1"}, {"value": "0.9", "module": "B2"}, {"value": "0.0", "module": "B3"}, {"value": "16.85", "module": "B4"}, {"value": "0.0", "module": "B5"}, {"value": "0.0", "module": "B6"}, {"value": "0.0", "module": "B7"}, {"value": "0.0", "module": "C1"}, {"value": "3.0", "module": "C2"}, {"value": "12.3", "module": "C3"}, {"value": "5.07", "module": "C4"}, {"value": "-72.25", "module": "D"}, {"name": "referenceToUnitGroupDataSet", "value": {"shortDescription": [{"value": "CTUe", "lang": "en"}], "type": "unit group data set", "refObjectId": "aa959ded-f1eb-4efb-9c5c-2d60be36b3e6", "version": "00.00.003", "uri": "../unitgroups/aa959ded-f1eb-4efb-9c5c-2d60be36b3e6.xml"}}]}}, {"referenceToLCIAMethodDataSet": {"shortDescription": [{"value": "Global Warming Potential - biogenic (GWP-biogenic)", "lang": "en"}, {"value": "Globales Erwärmungspotenzial - biogen (GWP-biogenic)", "lang": "de"}], "type": "LCIA method data set", "refObjectId": "a7ea186c-9749-11ed-a8fc-0242ac120002", "version": "01.00.006", "uri": "../lciamethods/a7ea186c-9749-11ed-a8fc-0242ac120002.xml"}, "meanAmount": 0.0, "other": {"anies": [{"value": "-9.37", "module": "A1-A3"}, {"value": "-0.19", "module": "A4"}, {"value": "8.81", "module": "A5"}, {"value": "0.0", "module": "B1"}, {"value": "-0.00155", "module": "B2"}, {"value": "0.0", "module": "B3"}, {"value": "-0.0177", "module": "B4"}, {"value": "0.0", "module": "B5"}, {"value": "0.0", "module": "B6"}, {"value": "0.0", "module": "B7"}, {"value": "0.0", "module": "C1"}, {"value": "-0.00399", "module": "C2"}, {"value": "0.038", "module": "C3"}, {"value": "-0.00162", "module": "C4"}, {"value": "-0.0959", "module": "D"}, {"name": "referenceToUnitGroupDataSet", "value": {"shortDescription": [{"value": "kg CO2-eq.", "lang": "en"}], "type": "unit group data set", "refObjectId": "1ebf3012-d0db-4de2-aefd-ef30cedb0be1", "version": "30.00.000", "uri": "../unitgroups/1ebf3012-d0db-4de2-aefd-ef30cedb0be1.xml"}}]}}, {"referenceToLCIAMethodDataSet": {"shortDescription": [{"value": "Global Warming Potential - fossil fuels (GWP-fossil)", "lang": "en"}, {"value": "Globales Erwärmungspotenzial - fossil (GWP-fossil)", "lang": "de"}], "type": "LCIA method data set", "refObjectId": "a7ea19c0-9749-11ed-a8fc-0242ac120002", "version": "01.00.009", "uri": "../lciamethods/a7ea19c0-9749-11ed-a8fc-0242ac120002.xml"}, "meanAmount": 0.0, "other": {"anies": [{"value": "143.4", "module": "A1-A3"}, {"value": "8.34", "module": "A4"}, {"value": "1.77", "module": "A5"}, {"value": "0.0", "module": "B1"}, {"value": "1.2", "module": "B2"}, {"value": "0.0", "module": "B3"}, {"value": "3.02", "module": "B4"}, {"value": "0.0", "module": "B5"}, {"value": "0.0", "module": "B6"}, {"value": "0.0", "module": "B7"}, {"value": "0.0", "module": "C1"}, {"value": "0.18", "module": "C2"}, {"value": "11.4", "module": "C3"}, {"value": "0.5", "module": "C4"}, {"value": "-46.6", "module": "D"}, {"name": "referenceToUnitGroupDataSet", "value": {"shortDescription": [{"value": "kg CO2-eq.", "lang": "en"}], "type": "unit group data set", "refObjectId": "1ebf3012-d0db-4de2-aefd-ef30cedb0be1", "version": "30.00.000", "uri": "../unitgroups/1ebf3012-d0db-4de2-aefd-ef30cedb0be1.xml"}}]}}, {"referenceToLCIAMethodDataSet": {"shortDescription": [{"value": "Global warming potential except emissions and uptake of biogenic carbon", "lang": "en"}], "type": "LCIA method data set", "refObjectId": "fb774615-0575-45de-9a89-1ded92f19770", "version": "01.00.000", "uri": "../lciamethods/fb774615-0575-45de-9a89-1ded92f19770.xml"}, "meanAmount": 0.0, "other": {"anies": [{"value": "143.77", "module": "A1-A3"}, {"value": "8.43", "module": "A4"}, {"value": "1.7899999999999991", "module": "A5"}, {"value": "0.0", "module": "B1"}, {"value": "1.20155", "module": "B2"}, {"value": "0.0", "module": "B3"}, {"value": "3.0277", "module": "B4"}, {"value": "0.0", "module": "B5"}, {"value": "0.0", "module": "B6"}, {"value": "0.0", "module": "B7"}, {"value": "0.0", "module": "C1"}, {"value": "0.18399", "module": "C2"}, {"value": "11.362", "module": "C3"}, {"value": "0.50162", "module": "C4"}, {"value": "-46.6041", "module": "D"}, {"name": "referenceToUnitGroupDataSet", "value": {"shortDescription": [{"value": "kg CO2-eq.", "lang": "en"}], "type": "unit group data set", "refObjectId": "1ebf3012-d0db-4de2-aefd-ef30cedb0be1", "version": "30.00.000", "uri": "../unitgroups/1ebf3012-d0db-4de2-aefd-ef30cedb0be1.xml"}}]}}, {"referenceToLCIAMethodDataSet": {"shortDescription": [{"value": "Global Warming Potential - land use and land use change (GWP-luluc)", "lang": "en"}, {"value": "Globales Erwärmungspotenzial - luluc (GWP-luluc)", "lang": "de"}], "type": "LCIA method data set", "refObjectId": "a7ea1ae2-9749-11ed-a8fc-0242ac120002", "version": "01.00.006", "uri": "../lciamethods/a7ea1ae2-9749-11ed-a8fc-0242ac120002.xml"}, "meanAmount": 0.0, "other": {"anies": [{"value": "0.4", "module": "A1-A3"}, {"value": "0.0858", "module": "A4"}, {"value": "2.14E-4", "module": "A5"}, {"value": "0.0", "module": "B1"}, {"value": "5.48E-4", "module": "B2"}, {"value": "0.0", "module": "B3"}, {"value": "0.00882", "module": "B4"}, {"value": "0.0", "module": "B5"}, {"value": "0.0", "module": "B6"}, {"value": "0.0", "module": "B7"}, {"value": "0.0", "module": "C1"}, {"value": "0.00186", "module": "C2"}, {"value": "0.00542", "module": "C3"}, {"value": "0.00205", "module": "C4"}, {"value": "-0.0674", "module": "D"}, {"name": "referenceToUnitGroupDataSet", "value": {"shortDescription": [{"value": "kg CO2-eq.", "lang": "en"}], "type": "unit group data set", "refObjectId": "1ebf3012-d0db-4de2-aefd-ef30cedb0be1", "version": "30.00.000", "uri": "../unitgroups/1ebf3012-d0db-4de2-aefd-ef30cedb0be1.xml"}}]}}, {"referenceToLCIAMethodDataSet": {"shortDescription": [{"value": "Global Warming Potential - total (GWP-total)", "lang": "en"}, {"value": "Globales Erwärmungspotenzial - total (GWP-total)", "lang": "de"}], "type": "LCIA method data set", "refObjectId": "a7ea142a-9749-11ed-a8fc-0242ac120002", "version": "04.00.017", "uri": "../lciamethods/a7ea142a-9749-11ed-a8fc-0242ac120002.xml"}, "meanAmount": 0.0, "other": {"anies": [{"value": "134.4", "module": "A1-A3"}, {"value": "8.24", "module": "A4"}, {"value": "10.6", "module": "A5"}, {"value": "0.0", "module": "B1"}, {"value": "1.2", "module": "B2"}, {"value": "0.0", "module": "B3"}, {"value": "3.01", "module": "B4"}, {"value": "0.0", "module": "B5"}, {"value": "0.0", "module": "B6"}, {"value": "0.0", "module": "B7"}, {"value": "0.0", "module": "C1"}, {"value": "0.18", "module": "C2"}, {"value": "11.4", "module": "C3"}, {"value": "0.5", "module": "C4"}, {"value": "-46.7", "module": "D"}, {"name": "referenceToUnitGroupDataSet", "value": {"shortDescription": [{"value": "kg CO2-eq.", "lang": "en"}], "type": "unit group data set", "refObjectId": "1ebf3012-d0db-4de2-aefd-ef30cedb0be1", "version": "30.00.000", "uri": "../unitgroups/1ebf3012-d0db-4de2-aefd-ef30cedb0be1.xml"}}]}}, {"referenceToLCIAMethodDataSet": {"shortDescription": [{"value": "Potential Comparative Toxic Unit for humans - cancer effects (HTP-c)", "lang": "en"}, {"value": "Potenzielle Toxizitätsvergleichseinheit für den Menschen - kanzerogene Wirkung (HTP-c)", "lang": "de"}], "type": "LCIA method data set", "refObjectId": "2299222a-bbd8-474f-9d4f-4dd1f18aea7c", "version": "01.00.004", "uri": "../lciamethods/2299222a-bbd8-474f-9d4f-4dd1f18aea7c.xml"}, "meanAmount": 0.0, "other": {"anies": [{"value": "6.39E-6", "module": "A1-A3"}, {"value": "1.87E-9", "module": "A4"}, {"value": "7.17E-11", "module": "A5"}, {"value": "0.0", "module": "B1"}, {"value": "1.27E-7", "module": "B2"}, {"value": "0.0", "module": "B3"}, {"value": "1.28E-7", "module": "B4"}, {"value": "0.0", "module": "B5"}, {"value": "0.0", "module": "B6"}, {"value": "0.0", "module": "B7"}, {"value": "0.0", "module": "C1"}, {"value": "4.05E-11", "module": "C2"}, {"value": "6.05E-10", "module": "C3"}, {"value": "8.72E-11", "module": "C4"}, {"value": "-3.83E-6", "module": "D"}, {"name": "referenceToUnitGroupDataSet", "value": {"shortDescription": [{"value": "CTUh", "lang": "en"}], "type": "unit group data set", "refObjectId": "d4c9523e-2d7e-49fd-8469-998f547d3a70", "version": "00.00.003", "uri": "../unitgroups/d4c9523e-2d7e-49fd-8469-998f547d3a70.xml"}}]}}, {"referenceToLCIAMethodDataSet": {"shortDescription": [{"value": "Potential Comparative Toxic Unit for humans - non-cancer effects (HTP-nc)", "lang": "en"}, {"value": "Potenzielle Toxizitätsvergleichseinheit für den Menschen - nicht kanzerogene Wirkung (HTP-nc)", "lang": "de"}], "type": "LCIA method data set", "refObjectId": "7cfdcfcf-b222-4b26-888a-a55f9fbf7ac8", "version": "01.00.003", "uri": "../lciamethods/7cfdcfcf-b222-4b26-888a-a55f9fbf7ac8.xml"}, "meanAmount": 0.0, "other": {"anies": [{"value": "7.56E-4", "module": "A1-A3"}, {"value": "1.05E-7", "module": "A4"}, {"value": "9.57E-10", "module": "A5"}, {"value": "0.0", "module": "B1"}, {"value": "1.51E-5", "module": "B2"}, {"value": "0.0", "module": "B3"}, {"value": "1.51E-5", "module": "B4"}, {"value": "0.0", "module": "B5"}, {"value": "0.0", "module": "B6"}, {"value": "0.0", "module": "B7"}, {"value": "0.0", "module": "C1"}, {"value": "2.27E-9", "module": "C2"}, {"value": "2.93E-8", "module": "C3"}, {"value": "3.26E-9", "module": "C4"}, {"value": "-4.54E-4", "module": "D"}, {"name": "referenceToUnitGroupDataSet", "value": {"shortDescription": [{"value": "CTUh", "lang": "en"}], "type": "unit group data set", "refObjectId": "d4c9523e-2d7e-49fd-8469-998f547d3a70", "version": "00.00.003", "uri": "../unitgroups/d4c9523e-2d7e-49fd-8469-998f547d3a70.xml"}}]}}, {"referenceToLCIAMethodDataSet": {"shortDescription": [{"value": "Potential Human exposure efficiency relative to U235 (IRP)", "lang": "en"}, {"value": "Potenzielle Wirkung durch Exposition des Menschen mit U235 (IRP)", "lang": "de"}], "type": "LCIA method data set", "refObjectId": "b5c632be-def3-11e6-bf01-fe55135034f3", "version": "01.00.012", "uri": "../lciamethods/b5c632be-def3-11e6-bf01-fe55135034f3.xml"}, "meanAmount": 0.0, "other": {"anies": [{"value": "4.0", "module": "A1-A3"}, {"value": "0.0289", "module": "A4"}, {"value": "0.0165", "module": "A5"}, {"value": "0.0", "module": "B1"}, {"value": "0.0336", "module": "B2"}, {"value": "0.0", "module": "B3"}, {"value": "0.0564", "module": "B4"}, {"value": "0.0", "module": "B5"}, {"value": "0.0", "module": "B6"}, {"value": "0.0", "module": "B7"}, {"value": "0.0", "module": "C1"}, {"value": "6.26E-4", "module": "C2"}, {"value": "0.54", "module": "C3"}, {"value": "0.00768", "module": "C4"}, {"value": "-2.74", "module": "D"}, {"name": "referenceToUnitGroupDataSet", "value": {"shortDescription": [{"value": "kgBq U235-eq.", "lang": "en"}], "type": "unit group data set", "refObjectId": "456b05bf-1415-44a9-9993-02452f554c09", "version": "00.00.003", "uri": "../unitgroups/456b05bf-1415-44a9-9993-02452f554c09.xml"}}]}}, {"referenceToLCIAMethodDataSet": {"shortDescription": [{"value": "Depletion potential of the stratospheric ozone layer (ODP)", "lang": "en"}, {"value": "Abbaupotenzial der stratosphärischen Ozonschicht (ODP)", "lang": "de"}], "type": "LCIA method data set", "refObjectId": "b5c629d6-def3-11e6-bf01-fe55135034f3", "version": "02.00.013", "uri": "../lciamethods/b5c629d6-def3-11e6-bf01-fe55135034f3.xml"}, "meanAmount": 0.0, "other": {"anies": [{"value": "4.59E-9", "module": "A1-A3"}, {"value": "1.38E-12", "module": "A4"}, {"value": "1.42E-12", "module": "A5"}, {"value": "0.0", "module": "B1"}, {"value": "6.78E-11", "module": "B2"}, {"value": "0.0", "module": "B3"}, {"value": "9.02E-11", "module": "B4"}, {"value": "0.0", "module": "B5"}, {"value": "0.0", "module": "B6"}, {"value": "0.0", "module": "B7"}, {"value": "0.0", "module": "C1"}, {"value": "2.99E-14", "module": "C2"}, {"value": "2.73E-11", "module": "C3"}, {"value": "1.39E-12", "module": "C4"}, {"value": "-1.82E-10", "module": "D"}, {"name": "referenceToUnitGroupDataSet", "value": {"shortDescription": [{"value": "kg CFC-11-eq.", "lang": "en"}], "type": "unit group data set", "refObjectId": "d9e957c9-7309-4474-bf3a-7777df6c4e5b", "version": "25.00.000", "uri": "../unitgroups/d9e957c9-7309-4474-bf3a-7777df6c4e5b.xml"}}]}}, {"referenceToLCIAMethodDataSet": {"shortDescription": [{"value": "Potential incidence of disease due to PM emissions (PM)", "lang": "en"}, {"value": "Potenzielles Auftreten von Krankheiten aufgrund von Feinstaubemissionen (PM)", "lang": "de"}], "type": "LCIA method data set", "refObjectId": "b5c602c6-def3-11e6-bf01-fe55135034f3", "version": "02.00.012", "uri": "../lciamethods/b5c602c6-def3-11e6-bf01-fe55135034f3.xml"}, "meanAmount": 0.0, "other": {"anies": [{"value": "6.25E-6", "module": "A1-A3"}, {"value": "1.59E-7", "module": "A4"}, {"value": "1.24E-8", "module": "A5"}, {"value": "0.0", "module": "B1"}, {"value": "7.1E-8", "module": "B2"}, {"value": "0.0", "module": "B3"}, {"value": "1.21E-7", "module": "B4"}, {"value": "0.0", "module": "B5"}, {"value": "0.0", "module": "B6"}, {"value": "0.0", "module": "B7"}, {"value": "0.0", "module": "C1"}, {"value": "2.34E-9", "module": "C2"}, {"value": "5.83E-8", "module": "C3"}, {"value": "4.4E-8", "module": "C4"}, {"value": "-2.48E-6", "module": "D"}, {"name": "referenceToUnitGroupDataSet", "value": {"shortDescription": [{"value": "Disease incidence", "lang": "en"}], "type": "unit group data set", "refObjectId": "3883559b-648f-4afc-8ba2-0bd24f3affa3", "version": "00.00.003", "uri": "../unitgroups/3883559b-648f-4afc-8ba2-0bd24f3affa3.xml"}}]}}, {"referenceToLCIAMethodDataSet": {"shortDescription": [{"value": "Photochemical Ozone Creation Potential (POCP)", "lang": "en"}, {"value": "Bildungspotenzial für troposphärisches Ozon (POCP)", "lang": "de"}], "type": "LCIA method data set", "refObjectId": "b5c610fe-def3-11e6-bf01-fe55135034f3", "version": "02.00.015", "uri": "../lciamethods/b5c610fe-def3-11e6-bf01-fe55135034f3.xml"}, "meanAmount": 0.0, "other": {"anies": [{"value": "0.28", "module": "A1-A3"}, {"value": "0.0179", "module": "A4"}, {"value": "0.00196", "module": "A5"}, {"value": "0.0", "module": "B1"}, {"value": "0.00214", "module": "B2"}, {"value": "0.0", "module": "B3"}, {"value": "0.00559", "module": "B4"}, {"value": "0.0", "module": "B5"}, {"value": "0.0", "module": "B6"}, {"value": "0.0", "module": "B7"}, {"value": "0.0", "module": "C1"}, {"value": "2.25E-4", "module": "C2"}, {"value": "0.00336", "module": "C3"}, {"value": "0.00276", "module": "C4"}, {"value": "-0.0867", "module": "D"}, {"name": "referenceToUnitGroupDataSet", "value": {"shortDescription": [{"value": "kg NMVOC-eq.", "lang": "en"}], "type": "unit group data set", "refObjectId": "d27c25f8-fbc1-44c6-b47b-4adbae4199c6", "version": "00.00.003", "uri": "../unitgroups/d27c25f8-fbc1-44c6-b47b-4adbae4199c6.xml"}}]}}, {"referenceToLCIAMethodDataSet": {"shortDescription": [{"value": "Potential Soil quality index (SQP)", "lang": "en"}, {"value": "Potenzieller Bodenqualitätsindex (SQP)", "lang": "de"}], "type": "LCIA method data set", "refObjectId": "b2ad6890-c78d-11e6-9d9d-cec0c932ce01", "version": "01.00.011", "uri": "../lciamethods/b2ad6890-c78d-11e6-9d9d-cec0c932ce01.xml"}, "meanAmount": 0.0, "other": {"anies": [{"value": "1879.3", "module": "A1-A3"}, {"value": "47.2", "module": "A4"}, {"value": "0.8", "module": "A5"}, {"value": "0.0", "module": "B1"}, {"value": "3.32", "module": "B2"}, {"value": "0.0", "module": "B3"}, {"value": "38.17", "module": "B4"}, {"value": "0.0", "module": "B5"}, {"value": "0.0", "module": "B6"}, {"value": "0.0", "module": "B7"}, {"value": "0.0", "module": "C1"}, {"value": "1.02", "module": "C2"}, {"value": "10.3", "module": "C3"}, {"value": "1.62", "module": "C4"}, {"value": "-93.2", "module": "D"}, {"name": "referenceToUnitGroupDataSet", "value": {"shortDescription": [{"value": "dimensionless", "lang": "en"}], "type": "unit group data set", "refObjectId": "f130951c-e67f-4f7f-8dd4-665de3974e18", "version": "00.00.004", "uri": "../unitgroups/f130951c-e67f-4f7f-8dd4-665de3974e18.xml"}}]}}, {"referenceToLCIAMethodDataSet": {"shortDescription": [{"value": "Water (user) deprivation potential (WDP)", "lang": "en"}, {"value": "Wasser-Entzugspotenzial (Benutzer) (WDP)", "lang": "de"}], "type": "LCIA method data set", "refObjectId": "b2ad66ce-c78d-11e6-9d9d-cec0c932ce01", "version": "03.00.015", "uri": "../lciamethods/b2ad66ce-c78d-11e6-9d9d-cec0c932ce01.xml"}, "meanAmount": 0.0, "other": {"anies": [{"value": "8.56", "module": "A1-A3"}, {"value": "0.0381", "module": "A4"}, {"value": "1.15", "module": "A5"}, {"value": "0.0", "module": "B1"}, {"value": "0.13", "module": "B2"}, {"value": "0.0", "module": "B3"}, {"value": "0.18", "module": "B4"}, {"value": "0.0", "module": "B5"}, {"value": "0.0", "module": "B6"}, {"value": "0.0", "module": "B7"}, {"value": "0.0", "module": "C1"}, {"value": "8.25E-4", "module": "C2"}, {"value": "1.26", "module": "C3"}, {"value": "0.054", "module": "C4"}, {"value": "-2.2", "module": "D"}, {"name": "referenceToUnitGroupDataSet", "value": {"shortDescription": [{"value": "m3 world eq. deprived", "lang": "en"}], "type": "unit group data set", "refObjectId": "6ae2df01-888e-46c8-b17d-49fa3869b476", "version": "00.00.003", "uri": "../unitgroups/6ae2df01-888e-46c8-b17d-49fa3869b476.xml"}}]}}]}, "otherAttributes": {"{http://www.indata.network/EPD/2019}epd-version": "1.2", "{http://www.okworx.com/ILCD/Extensions/2018/Profile}profile": "EN_15804_A2"}, "version": "1.1"}