{"processInformation": {"dataSetInformation": {"UUID": "299cd856-c220-4b82-910d-60c91e035c7d", "name": {"baseName": [{"value": "Access manager 92 90 Wall", "lang": "en"}, {"value": "Access manager 92 90 Wall", "lang": "de"}], "functionalUnitFlowProperties": [{"lang": "en"}]}, "classificationInformation": {"classification": [{"class": [{"value": "Gebäudetechnik", "level": 0, "classId": "8"}, {"value": "Elektro", "level": 1, "classId": "8.4"}, {"value": "Sicherungs- und Schaltschränke", "level": 2, "classId": "8.4.03"}], "name": "OEKOBAU.DAT"}, {"class": [{"value": "02 Building products", "level": 0}, {"value": "Doors, windows, shutters, and related products", "level": 1}, {"value": "Electronic and physical Access Control Systems", "level": 2}], "name": "IBUCategories"}]}, "generalComment": [{"value": "The dormakaba access manager 92 90 as a central access control manager meets all the requirements of modern access control. Thanks to its intelligent decision logic and free parametrisation, it controls all access events, at basic access points as well as to complex, highly sensitive company areas. Predefined configurations simplify the setting of individual door functions. The state-of-the-art IT security is based on a modern operating system and TLS (Transport Layer Security) encryption that can be activated between controller and host system: the control electronics integrates all the necessary requirements to enable a connection to Cloud Services via IoT. Therefore, the access manager 92 90 is already designed for the requirements of tomorrow.\nSwitching to other dormakaba access solutions at a later point is also possible.", "lang": "en"}, {"value": "Der dormakaba access manager 92 90 erfüllt als zentraler Zutrittskontrollmanager alle Anforderungen an eine moderne Zutrittskontrolle. Dank seiner intelligenten Entscheidungslogik und der freien Parametrierung steuert er alle Zutrittsereignisse, sowohl an einfachen Zugängen als auch zu komplexen, hochsensiblen Unternehmensbereichen. Vordefinierte Konfigurationen vereinfachen die Einstellung der einzelnen Türfunktionen. Die hochmoderne IT-Sicherheit basiert auf einem modernen Betriebssystem und einer TLS-Verschlüsselung (Transport Layer Security), die zwischen Controller und Hostsystem aktiviert werden kann: Die Steuerelektronik integriert alle notwendigen Voraussetzungen, um eine Verbindung zu Cloud Services über IoT zu ermöglichen. Der Zutrittsmanager 92 90 ist also schon heute für die Anforderungen von morgen ausgelegt. Ein späterer Wechsel zu anderen dormakaba Zutrittslösungen ist ebenfalls möglich.", "lang": "de"}]}, "quantitativeReference": {"referenceToReferenceFlow": [0]}, "time": {"referenceYear": 2021, "dataSetValidUntil": 2026, "other": {"anies": [{"name": "publicationDateOfEPD", "value": 1620691200000}]}}, "geography": {"locationOfOperationSupplyOrProduction": {"location": "DE"}}, "technology": {"technologyDescriptionAndIncludedProcesses": [{"value": "As a central access control manager, the dormakaba access manager 92 90 meets all the requirements of modern access control. Thanks to its intelligent decision logic and free parameterization, it controls all access events, both at simple access points and to complex, highly sensitive company areas. \nTechnical data: \nThe access manager 92 90 Wall has the following technical properties: \nDeclared unit: \nThe declared unit is 1 piece of the product: Access manager 92 90 Wall.", "lang": "en"}, {"value": "Der dormakaba access manager 92 90 erfüllt als zentraler Zutrittskontrollmanager alle Anforderungen an eine moderne Zutrittskontrolle. Dank seiner intelligenten Entscheidungslogik und der freien Parametrierung steuert er alle Zutrittsereignisse, sowohl an einfachen Zutrittspunkten als auch zu komplexen, hochsensiblen Unternehmensbereichen. \nTechnische Daten: \nDer Zugangsmanager 92 90 Wall hat die folgenden technischen Eigenschaften: \nDeklarierte Einheit: \nDie angegebene Einheit ist 1 Stück des Produkts: Access manager 92 90 Wall.", "lang": "de"}], "technologicalApplicability": [{"value": "Central Access control\nAn access manager is installed in a protected environment and uses various test criteria to check whether a booking made on a reader is authorized or not.\n\nDoor management\n• Personnel interlock control\n• Door activation\n• Monitoring of door opening\n• Monitoring of door opening time\n• Access monitoring\n\nAlarm Management\nThe access manager reports irregularities in access control or door management to the host computer. An additional function is to activate relays.", "lang": "en"}, {"value": "Zentrale Zutrittskontrolle Ein Zutrittsmanager wird in einer geschützten Umgebung installiert und prüft anhand verschiedener Prüfkriterien, ob eine an einem Leser vorgenommene Buchung berechtigt ist oder nicht. Türmanagement - Personenschleusensteuerung - Türaktivierung - Überwachung der Türöffnung - Überwachung der Türöffnungszeit - Zutrittsüberwachung Alarmmanagement Der Zutrittsmanager meldet Unregelmäßigkeiten bei der Zutrittskontrolle oder dem Türmanagement an den Hostcomputer. Eine weitere Funktion ist die Aktivierung von Relais.", "lang": "de"}]}}, "modellingAndValidation": {"LCIMethodAndAllocation": {"typeOfDataSet": "EPD", "referenceToLCAMethodDetails": [{"shortDescription": [{"value": "Electronic and physical Access Control Systems.pdf", "lang": "en"}], "type": "source data set", "refObjectId": "4e1eb9f7-bfc8-4851-8818-9e2e4dba7c4c"}], "other": {"anies": [{"name": "subType", "value": "specific dataset"}]}}, "dataSourcesTreatmentAndRepresentativeness": {"referenceToDataSource": [{"shortDescription": [{"value": "GaBi Database (all versions)", "lang": "en"}], "type": "source data set", "refObjectId": "28d74cc0-db8b-4d7e-bc44-5f6d56ce0c4a"}, {"shortDescription": [{"value": "GaBi database SP40 2020", "lang": "en"}], "type": "source data set", "refObjectId": "0115289e-52f0-4920-bc7e-57b1c96aec8d"}], "useAdviceForDataSet": [{"value": "Scope: \nThis EPD refers to a specific product manufactured by dormakaba. The production site is located in Villingen-Schwenningen (Germany), and the year of data collection is 2019. \nSystem boundary: \nThe type of EPD is: cradle to gate with options, modules C1–C4, and module D (A1–A3 + C + D and additional modules: A4 + A5 + B6) Production - Module A1-A3\nThe product stage includes:\n— A1, raw material extraction, processing and mechanical treatments, processing of secondary material input (e.g. recycling processes), — A2, transport to the manufacturer, — A3, manufacturing and assembly including provision of all materials, products and energy, as well as waste processing up to the end-of waste state.\n\nConstruction stage - Modules A4-A5\nThe construction process stage includes:\n— A4, transport to the building site; — A5, installation into the building; including provision of all materials, products and energy, as well as waste processing up to the end-of-waste state or disposal of final residues during the construction process stage.\n\nUse stage - Module B6\nThe use stage related to the operation of the building includes:\n— B6, operational energy use\n\nEnd-of-life stage– Modules C1-C4 and D\nThe end-of-life stage includes:\n— C1, de-construction, demolition:\n— C2, transport to waste processing; — C3, waste processing for reuse, recovery and/or recycling;\n— C4, disposal;\n\nincluding provision and all transport, provision of all materials, products and related energy and water use.\n\nModule D (Benefits and loads beyond the system boundary) includes:\n— D, recycling potentials, expressed as net impacts and benefits.", "lang": "en"}, {"value": "Gültigkeitsbereich: \nDiese EPD bezieht sich auf ein bestimmtes Produkt, das von dormakaba hergestellt wird. Die Produktionsstätte befindet sich in Villingen-Schwenningen (Deutschland), und das Jahr der Datenerhebung ist 2019. \nSystemgrenze: \nDie Art der EPD ist: Cradle to Gate mit Optionen, Modulen C1-C4 und Modul D (A1-A3 + C + D und zusätzliche Module: A4 + A5 + B6) Produktion - Modul A1-A3 Die Produktphase umfasst: - A1, Rohstoffgewinnung, Verarbeitung und mechanische Behandlungen, Verarbeitung von Sekundärmaterialinput (z.B. Recyclingprozesse), - A2, Transport zum Hersteller, - A3, Herstellung und Montage einschließlich Bereitstellung aller Materialien, Produkte und Energie sowie Abfallverarbeitung bis zum End-of-Waste-Zustand.\n\nBauphase - Module A4-A5 Die Bauprozessphase umfasst: - A4, Transport zur Baustelle; - A5, Einbau in das Gebäude; einschließlich der Bereitstellung aller Materialien, Produkte und Energie sowie der Abfallverarbeitung bis zum Abfallende oder der Entsorgung der letzten Rückstände während der Bauprozessphase.\n\nNutzungsphase - Modul B6 Die Nutzungsphase im Zusammenhang mit dem Betrieb des Gebäudes umfasst: - B6, betrieblicher Energieverbrauch End-of-Life-Phase - Module C1-C4 und D Die End-of-Life-Phase umfasst: - C1, Rückbau, Abriss; - C2, Transport zur Abfallverarbeitung; - C3, Abfallverarbeitung zur Wiederverwendung, Verwertung und/oder zum Recycling; - C4, Entsorgung; einschließlich Bereitstellung und sämtlicher Transporte, Bereitstellung aller Materialien, Produkte und des damit verbundenen Energie- und Wasserverbrauchs. Modul D (Nutzen und Belastungen jenseits der Systemgrenze) umfasst: - D, Recyclingpotenziale, ausgedrückt als Nettoauswirkungen und Nutzen.", "lang": "de"}], "other": {"anies": [{"name": "referenceToOriginalEPD", "value": {"shortDescription": {"value": "Access manager 92 90 Wall.pdf", "defaultValue": "Access manager 92 90 Wall.pdf", "lstrings": [{"lang": "en", "value": "Access manager 92 90 Wall.pdf"}]}, "type": "source data set", "uuid": {"uuid": "027c14f6-0be4-4e8b-ab59-7b6e7d8ef8c4"}, "refObjectId": "027c14f6-0be4-4e8b-ab59-7b6e7d8ef8c4", "resourceURLs": ["https://oekobaudat.de/OEKOBAU.DAT/resource/sources/027c14f6-0be4-4e8b-ab59-7b6e7d8ef8c4/Access_manager_92_90_Wall_22652.pdf?version=00.04.000"]}}]}}, "validation": {"review": [{"referenceToNameOfReviewerAndInstitution": [{"shortDescription": [{"value": "Institut Bauen und Umwelt e. V.", "lang": "en"}], "type": "contact data set", "refObjectId": "d111dbec-b024-4be5-86c5-752d6eb2cf95", "uri": "../contacts/d111dbec-b024-4be5-86c5-752d6eb2cf95.xml"}], "type": "Accredited third party review"}]}, "complianceDeclarations": {"compliance": [{"referenceToComplianceSystem": {"shortDescription": [{"value": "DIN EN 15804+A2", "lang": "en"}], "type": "source data set", "refObjectId": "c0016b33-8cf7-415c-ac6e-deba0d21440d", "uri": "../sources/c0016b33-8cf7-415c-ac6e-deba0d21440d.xml"}}, {"referenceToComplianceSystem": {"shortDescription": [{"value": "ISO 14025", "lang": "en"}], "type": "source data set", "refObjectId": "4f2eb655-6e44-4874-a95a-e28f5442cd4d", "uri": "../sources/4f2eb655-6e44-4874-a95a-e28f5442cd4d.xml"}}]}}, "administrativeInformation": {"commissionerAndGoal": {"referenceToCommissioner": [{"shortDescription": [{"value": "dormakaba International Holding GmbH", "lang": "en"}], "type": "contact data set", "refObjectId": "33313944-7b37-498a-b458-25a295c1017d", "uri": "../contacts/33313944-7b37-498a-b458-25a295c1017d.xml"}]}, "dataGenerator": {"referenceToPersonOrEntityGeneratingTheDataSet": [{"shortDescription": [{"value": "Sphera Solutions GmbH", "lang": "en"}], "type": "contact data set", "refObjectId": "623edf96-39d1-4e6f-9892-674c7228546b", "uri": "../contacts/623edf96-39d1-4e6f-9892-674c7228546b.xml"}]}, "dataEntryBy": {"timeStamp": 1620691200000, "referenceToDataSetFormat": [{"shortDescription": [{"value": "ILCD Format", "lang": "en"}], "type": "source data set", "refObjectId": "a97a0155-0234-4b87-b4ce-a45da52f2a40", "uri": "../sources/a97a0155-0234-4b87-b4ce-a45da52f2a40.xml"}, {"shortDescription": [{"value": "EPD-Datenformaterweiterungen v1.2", "lang": "de"}, {"value": "EPD Data Format Extensions v1.2", "lang": "en"}], "type": "source data set", "refObjectId": "a29449fd-aa2f-4de8-b5d7-4b06b43c6fde", "uri": "../sources/a29449fd-aa2f-4de8-b5d7-4b06b43c6fde.xml"}]}, "publicationAndOwnership": {"dataSetVersion": "00.06.000", "referenceToRegistrationAuthority": {"shortDescription": [{"value": "Institut Bauen und Umwelt e. V.", "lang": "en"}], "type": "contact data set", "refObjectId": "d111dbec-b024-4be5-86c5-752d6eb2cf95", "uri": "../contacts/d111dbec-b024-4be5-86c5-752d6eb2cf95.xml"}, "registrationNumber": "EPD-DOR-20210012-CCA2-EN", "referenceToOwnershipOfDataSet": {"shortDescription": [{"value": "dormakaba International Holding GmbH", "lang": "en"}], "type": "contact data set", "refObjectId": "33313944-7b37-498a-b458-25a295c1017d", "uri": "../contacts/33313944-7b37-498a-b458-25a295c1017d.xml"}, "copyright": true, "licenseType": "Free of charge for all users and uses", "accessRestrictions": [{"value": "None", "lang": "en"}], "other": {"anies": [{"name": "referenceToPublisher", "value": {"shortDescription": [{"value": "Institut Bauen und Umwelt e. V.", "lang": "en"}], "type": "contact data set", "refObjectId": "d111dbec-b024-4be5-86c5-752d6eb2cf95", "uri": "../contacts/d111dbec-b024-4be5-86c5-752d6eb2cf95.xml"}}]}}}, "exchanges": {"exchange": [{"dataSetInternalID": 0, "referenceToFlowDataSet": {"shortDescription": [{"value": "Access manager 92 90 Wall (Access manager 92 90 Wall)", "lang": "en"}], "type": "flow data set", "refObjectId": "f761715f-bf44-2722-5f56-539a4aa8f760", "uri": "../flows/f761715f-bf44-2722-5f56-539a4aa8f760.xml"}, "meanAmount": 1.0, "referencesToDataSource": {}, "referenceFlow": true, "resolvedFlowVersion": "00.05.000", "resultingflowAmount": 1.0, "flowProperties": [{"name": [{"lang": "de", "value": "Anzahl"}, {"lang": "en", "value": "Number of pieces"}], "uuid": "01846770-4cfe-4a25-8ad9-919d8d378345", "referenceFlowProperty": true, "meanValue": 1.0, "referenceUnit": "pcs.", "unitGroupUUID": "934110e3-baf4-49e9-992c-3d8109a6aafb"}], "materialProperties": [{"name": "weight per piece", "value": "11.676", "unit": "kg"}], "typeOfFlow": "Product flow", "classification": {"classHierarchy": "Komponenten von Fenstern und Vorhangfassaden / Türen und Tore / Stahl", "name": "OEKOBAU.DAT"}}, {"dataSetInternalID": 1, "referenceToFlowDataSet": {"shortDescription": [{"value": "Renewable primary energy as energy carrier (PERE)", "lang": "en"}, {"value": "Erneuerbare Primärenergie als Energieträger (PERE)", "lang": "de"}], "type": "flow data set", "refObjectId": "20f32be5-0398-4288-9b6d-accddd195317", "uri": "../flows/20f32be5-0398-4288-9b6d-accddd195317.xml"}, "exchange direction": "INPUT", "other": {"anies": [{"name": "referenceToUnitGroupDataSet", "value": {"shortDescription": [{"value": "MJ", "lang": "en"}], "type": "unit group data set", "refObjectId": "93a60a57-a3c8-11da-a746-0800200c9a66", "uri": "../unitgroups/93a60a57-a3c8-11da-a746-0800200c9a66.xml"}}, {"value": "156.20467", "module": "A1-A3"}, {"value": "0.00436", "module": "A4"}, {"value": "26.6", "module": "A5"}, {"value": "2540", "module": "B6"}, {"value": "0", "module": "C1"}, {"value": "0.00164", "module": "C2"}, {"value": "0.0316", "module": "C3"}, {"value": "0.0479", "module": "C4"}, {"value": "-6.31", "module": "D"}]}, "resolvedFlowVersion": "38.00.000", "flowProperties": [], "typeOfFlow": "Other flow", "classification": {"classHierarchy": "Quantities", "name": "GaBiCategories"}}, {"dataSetInternalID": 2, "referenceToFlowDataSet": {"shortDescription": [{"value": "Renewable primary energy resources as material utilization (PERM)", "lang": "en"}, {"value": "Erneuerbare Primärenergie zur stofflichen Nutzung (PERM)", "lang": "de"}], "type": "flow data set", "refObjectId": "fb3ec0de-548d-4508-aea5-00b73bf6f702", "uri": "../flows/fb3ec0de-548d-4508-aea5-00b73bf6f702.xml"}, "exchange direction": "INPUT", "other": {"anies": [{"name": "referenceToUnitGroupDataSet", "value": {"shortDescription": [{"value": "MJ", "lang": "en"}], "type": "unit group data set", "refObjectId": "93a60a57-a3c8-11da-a746-0800200c9a66", "uri": "../unitgroups/93a60a57-a3c8-11da-a746-0800200c9a66.xml"}}, {"value": "26.4143", "module": "A1-A3"}, {"value": "0", "module": "A4"}, {"value": "-26.4", "module": "A5"}, {"value": "0", "module": "B6"}, {"value": "0", "module": "C1"}, {"value": "0", "module": "C2"}, {"value": "-0.0143", "module": "C3"}, {"value": "0", "module": "C4"}, {"value": "0", "module": "D"}]}, "resolvedFlowVersion": "38.00.000", "flowProperties": [], "typeOfFlow": "Other flow", "classification": {"classHierarchy": "Quantities", "name": "GaBiCategories"}}, {"dataSetInternalID": 3, "referenceToFlowDataSet": {"shortDescription": [{"value": "Total use of renewable primary energy resources (PERT)", "lang": "en"}, {"value": "Total erneuerbare Primärenergie (PERT)", "lang": "de"}], "type": "flow data set", "refObjectId": "53f97275-fa8a-4cdd-9024-65936002acd0", "uri": "../flows/53f97275-fa8a-4cdd-9024-65936002acd0.xml"}, "exchange direction": "INPUT", "other": {"anies": [{"name": "referenceToUnitGroupDataSet", "value": {"shortDescription": [{"value": "MJ", "lang": "en"}], "type": "unit group data set", "refObjectId": "93a60a57-a3c8-11da-a746-0800200c9a66", "uri": "../unitgroups/93a60a57-a3c8-11da-a746-0800200c9a66.xml"}}, {"value": "182.61467", "module": "A1-A3"}, {"value": "0.00436", "module": "A4"}, {"value": "0.185", "module": "A5"}, {"value": "2540", "module": "B6"}, {"value": "0", "module": "C1"}, {"value": "0.00164", "module": "C2"}, {"value": "0.0173", "module": "C3"}, {"value": "0.0479", "module": "C4"}, {"value": "-6.31", "module": "D"}]}, "resolvedFlowVersion": "38.00.000", "flowProperties": [], "typeOfFlow": "Other flow", "classification": {"classHierarchy": "Quantities / Environmental quantities / EPD EN 15804 / LCI indicators", "name": "GaBiCategories"}}, {"dataSetInternalID": 4, "referenceToFlowDataSet": {"shortDescription": [{"value": "Non renewable primary energy as energy carrier (PENRE)", "lang": "en"}, {"value": "Nicht-erneuerbare Primärenergie als Energieträger (PENRE)", "lang": "de"}], "type": "flow data set", "refObjectId": "ac857178-2b45-46ec-892a-a9a4332f0372", "uri": "../flows/ac857178-2b45-46ec-892a-a9a4332f0372.xml"}, "exchange direction": "INPUT", "other": {"anies": [{"name": "referenceToUnitGroupDataSet", "value": {"shortDescription": [{"value": "MJ", "lang": "en"}], "type": "unit group data set", "refObjectId": "93a60a57-a3c8-11da-a746-0800200c9a66", "uri": "../unitgroups/93a60a57-a3c8-11da-a746-0800200c9a66.xml"}}, {"value": "604.36", "module": "A1-A3"}, {"value": "1.39", "module": "A4"}, {"value": "1.87", "module": "A5"}, {"value": "5740", "module": "B6"}, {"value": "0", "module": "C1"}, {"value": "0.52", "module": "C2"}, {"value": "6.45", "module": "C3"}, {"value": "0.366", "module": "C4"}, {"value": "-33.7", "module": "D"}]}, "resolvedFlowVersion": "38.00.000", "flowProperties": [], "typeOfFlow": "Other flow", "classification": {"classHierarchy": "Quantities", "name": "GaBiCategories"}}, {"dataSetInternalID": 5, "referenceToFlowDataSet": {"shortDescription": [{"value": "Non renewable primary energy as material utilization (PENRM)", "lang": "en"}, {"value": "Nicht-erneuerbare Primärenergie zur stofflichen Nutzung (PENRM)", "lang": "de"}], "type": "flow data set", "refObjectId": "1421caa0-679d-4bf4-b282-0eb850ccae27", "uri": "../flows/1421caa0-679d-4bf4-b282-0eb850ccae27.xml"}, "exchange direction": "INPUT", "other": {"anies": [{"name": "referenceToUnitGroupDataSet", "value": {"shortDescription": [{"value": "MJ", "lang": "en"}], "type": "unit group data set", "refObjectId": "93a60a57-a3c8-11da-a746-0800200c9a66", "uri": "../unitgroups/93a60a57-a3c8-11da-a746-0800200c9a66.xml"}}, {"value": "7.24", "module": "A1-A3"}, {"value": "0", "module": "A4"}, {"value": "-0.86", "module": "A5"}, {"value": "0", "module": "B6"}, {"value": "0", "module": "C1"}, {"value": "0", "module": "C2"}, {"value": "-6.38", "module": "C3"}, {"value": "0", "module": "C4"}, {"value": "0", "module": "D"}]}, "resolvedFlowVersion": "38.00.000", "flowProperties": [], "typeOfFlow": "Other flow", "classification": {"classHierarchy": "Quantities", "name": "GaBiCategories"}}, {"dataSetInternalID": 6, "referenceToFlowDataSet": {"shortDescription": [{"value": "Total use of non renewable primary energy resources (PENRT)", "lang": "en"}, {"value": "Total nicht erneuerbare Primärenergie (PENRT)", "lang": "de"}], "type": "flow data set", "refObjectId": "06159210-646b-4c8d-8583-da9b3b95a6c1", "uri": "../flows/06159210-646b-4c8d-8583-da9b3b95a6c1.xml"}, "exchange direction": "INPUT", "other": {"anies": [{"name": "referenceToUnitGroupDataSet", "value": {"shortDescription": [{"value": "MJ", "lang": "en"}], "type": "unit group data set", "refObjectId": "93a60a57-a3c8-11da-a746-0800200c9a66", "uri": "../unitgroups/93a60a57-a3c8-11da-a746-0800200c9a66.xml"}}, {"value": "612.22", "module": "A1-A3"}, {"value": "1.39", "module": "A4"}, {"value": "1.01", "module": "A5"}, {"value": "5740", "module": "B6"}, {"value": "0", "module": "C1"}, {"value": "0.52", "module": "C2"}, {"value": "0.0667", "module": "C3"}, {"value": "0.366", "module": "C4"}, {"value": "-33.7", "module": "D"}]}, "resolvedFlowVersion": "38.00.000", "flowProperties": [], "typeOfFlow": "Other flow", "classification": {"classHierarchy": "Quantities / Environmental quantities / EPD EN 15804 / LCI indicators", "name": "GaBiCategories"}}, {"dataSetInternalID": 7, "referenceToFlowDataSet": {"shortDescription": [{"value": "Use of secondary material (SM)", "lang": "en"}, {"value": "Einsatz von Sekundärstoffen (SM)", "lang": "de"}], "type": "flow data set", "refObjectId": "c6a1f35f-2d09-4f54-8dfb-97e502e1ce92", "uri": "../flows/c6a1f35f-2d09-4f54-8dfb-97e502e1ce92.xml"}, "exchange direction": "INPUT", "other": {"anies": [{"name": "referenceToUnitGroupDataSet", "value": {"shortDescription": [{"value": "kg", "lang": "en"}], "type": "unit group data set", "refObjectId": "ad38d542-3fe9-439d-9b95-2f5f7752acaf", "uri": "../unitgroups/ad38d542-3fe9-439d-9b95-2f5f7752acaf.xml"}}, {"value": "7.49", "module": "A1-A3"}, {"value": "0", "module": "A4"}, {"value": "0", "module": "A5"}, {"value": "0", "module": "B6"}, {"value": "0", "module": "C1"}, {"value": "0", "module": "C2"}, {"value": "0", "module": "C3"}, {"value": "0", "module": "C4"}, {"value": "0", "module": "D"}]}, "resolvedFlowVersion": "38.00.000", "flowProperties": [], "typeOfFlow": "Other flow", "classification": {"classHierarchy": "Quantities / Environmental quantities / EPD EN 15804 / LCI indicators", "name": "GaBiCategories"}}, {"dataSetInternalID": 8, "referenceToFlowDataSet": {"shortDescription": [{"value": "Use of renewable secondary fuels (RSF)", "lang": "en"}, {"value": "Erneuerbare Sekundärbrennstoffe (RSF)", "lang": "de"}], "type": "flow data set", "refObjectId": "64333088-a55f-4aa2-9a31-c10b07816787", "uri": "../flows/64333088-a55f-4aa2-9a31-c10b07816787.xml"}, "exchange direction": "INPUT", "other": {"anies": [{"name": "referenceToUnitGroupDataSet", "value": {"shortDescription": [{"value": "MJ", "lang": "en"}], "type": "unit group data set", "refObjectId": "93a60a57-a3c8-11da-a746-0800200c9a66", "uri": "../unitgroups/93a60a57-a3c8-11da-a746-0800200c9a66.xml"}}, {"value": "0", "module": "A1-A3"}, {"value": "0", "module": "A4"}, {"value": "0", "module": "A5"}, {"value": "0", "module": "B6"}, {"value": "0", "module": "C1"}, {"value": "0", "module": "C2"}, {"value": "0", "module": "C3"}, {"value": "0", "module": "C4"}, {"value": "0", "module": "D"}]}, "resolvedFlowVersion": "38.00.000", "flowProperties": [], "typeOfFlow": "Other flow", "classification": {"classHierarchy": "Quantities / Environmental quantities / EPD EN 15804 / LCI indicators", "name": "GaBiCategories"}}, {"dataSetInternalID": 9, "referenceToFlowDataSet": {"shortDescription": [{"value": "Use of non renewable secondary fuels (NRSF)", "lang": "en"}, {"value": "Nicht erneuerbare Sekundärbrennstoffe (NRSF)", "lang": "de"}], "type": "flow data set", "refObjectId": "89def144-d39a-4287-b86f-efde453ddcb2", "uri": "../flows/89def144-d39a-4287-b86f-efde453ddcb2.xml"}, "exchange direction": "INPUT", "other": {"anies": [{"name": "referenceToUnitGroupDataSet", "value": {"shortDescription": [{"value": "MJ", "lang": "en"}], "type": "unit group data set", "refObjectId": "93a60a57-a3c8-11da-a746-0800200c9a66", "uri": "../unitgroups/93a60a57-a3c8-11da-a746-0800200c9a66.xml"}}, {"value": "0", "module": "A1-A3"}, {"value": "0", "module": "A4"}, {"value": "0", "module": "A5"}, {"value": "0", "module": "B6"}, {"value": "0", "module": "C1"}, {"value": "0", "module": "C2"}, {"value": "0", "module": "C3"}, {"value": "0", "module": "C4"}, {"value": "0", "module": "D"}]}, "resolvedFlowVersion": "38.00.000", "flowProperties": [], "typeOfFlow": "Other flow", "classification": {"classHierarchy": "Quantities / Environmental quantities / EPD EN 15804 / LCI indicators", "name": "GaBiCategories"}}, {"dataSetInternalID": 10, "referenceToFlowDataSet": {"shortDescription": [{"value": "Use of net fresh water (FW)", "lang": "en"}, {"value": "Einsatz von Süßwasserressourcen (FW)", "lang": "de"}], "type": "flow data set", "refObjectId": "3cf952c8-f3a4-461d-8c96-96456ca62246", "uri": "../flows/3cf952c8-f3a4-461d-8c96-96456ca62246.xml"}, "exchange direction": "INPUT", "other": {"anies": [{"name": "referenceToUnitGroupDataSet", "value": {"shortDescription": [{"value": "m^3", "lang": "en"}], "type": "unit group data set", "refObjectId": "cd950537-0a98-4044-9ba7-9f9a68d0a504", "uri": "../unitgroups/cd950537-0a98-4044-9ba7-9f9a68d0a504.xml"}}, {"value": "0.32857838", "module": "A1-A3"}, {"value": "7.83E-06", "module": "A4"}, {"value": "0.00923", "module": "A5"}, {"value": "2.94", "module": "B6"}, {"value": "0", "module": "C1"}, {"value": "2.94E-06", "module": "C2"}, {"value": "0.000352", "module": "C3"}, {"value": "9.22E-05", "module": "C4"}, {"value": "-0.0165", "module": "D"}]}, "resolvedFlowVersion": "38.00.000", "flowProperties": [], "typeOfFlow": "Other flow", "classification": {"classHierarchy": "Quantities / Environmental quantities / EPD EN 15804 / LCI indicators", "name": "GaBiCategories"}}, {"dataSetInternalID": 11, "referenceToFlowDataSet": {"shortDescription": [{"value": "Hazardous waste disposed (HWD)", "lang": "en"}, {"value": "Gefährlicher Abfall zur Deponie (HWD)", "lang": "de"}], "type": "flow data set", "refObjectId": "430f9e0f-59b2-46a0-8e0d-55e0e84948fc", "uri": "../flows/430f9e0f-59b2-46a0-8e0d-55e0e84948fc.xml"}, "exchange direction": "OUTPUT", "other": {"anies": [{"name": "referenceToUnitGroupDataSet", "value": {"shortDescription": [{"value": "kg", "lang": "en"}], "type": "unit group data set", "refObjectId": "ad38d542-3fe9-439d-9b95-2f5f7752acaf", "uri": "../unitgroups/ad38d542-3fe9-439d-9b95-2f5f7752acaf.xml"}}, {"value": "2.8699752E-05", "module": "A1-A3"}, {"value": "1.34E-10", "module": "A4"}, {"value": "1.54E-09", "module": "A5"}, {"value": "2.37E-06", "module": "B6"}, {"value": "0", "module": "C1"}, {"value": "5.04E-11", "module": "C2"}, {"value": "2.54E-10", "module": "C3"}, {"value": "5.57E-09", "module": "C4"}, {"value": "1.06E-07", "module": "D"}]}, "resolvedFlowVersion": "38.00.000", "flowProperties": [], "typeOfFlow": "Other flow", "classification": {"classHierarchy": "Quantities / Environmental quantities / EPD EN 15804 / LCI indicators", "name": "GaBiCategories"}}, {"dataSetInternalID": 12, "referenceToFlowDataSet": {"shortDescription": [{"value": "Non hazardous waste disposed (NHWD)", "lang": "en"}, {"value": "Entsorgter nicht gefährlicher Abfall (NHWD)", "lang": "de"}], "type": "flow data set", "refObjectId": "b29ef66b-e286-4afa-949f-62f1a7b4d7fa", "uri": "../flows/b29ef66b-e286-4afa-949f-62f1a7b4d7fa.xml"}, "exchange direction": "OUTPUT", "other": {"anies": [{"name": "referenceToUnitGroupDataSet", "value": {"shortDescription": [{"value": "kg", "lang": "en"}], "type": "unit group data set", "refObjectId": "ad38d542-3fe9-439d-9b95-2f5f7752acaf", "uri": "../unitgroups/ad38d542-3fe9-439d-9b95-2f5f7752acaf.xml"}}, {"value": "3.108452", "module": "A1-A3"}, {"value": "0.000142", "module": "A4"}, {"value": "0.103", "module": "A5"}, {"value": "4.07", "module": "B6"}, {"value": "0", "module": "C1"}, {"value": "5.32E-05", "module": "C2"}, {"value": "0.0149", "module": "C3"}, {"value": "1.84", "module": "C4"}, {"value": "-0.336", "module": "D"}]}, "resolvedFlowVersion": "38.00.000", "flowProperties": [], "typeOfFlow": "Other flow", "classification": {"classHierarchy": "Quantities / Environmental quantities / EPD EN 15804 / LCI indicators", "name": "GaBiCategories"}}, {"dataSetInternalID": 13, "referenceToFlowDataSet": {"shortDescription": [{"value": "Radioactive waste disposed (RWD)", "lang": "en"}, {"value": "Entsorgter radioaktiver Abfall (RWD)", "lang": "de"}], "type": "flow data set", "refObjectId": "3449546e-52ad-4b39-b809-9fb77cea8ff6", "uri": "../flows/3449546e-52ad-4b39-b809-9fb77cea8ff6.xml"}, "exchange direction": "OUTPUT", "other": {"anies": [{"name": "referenceToUnitGroupDataSet", "value": {"shortDescription": [{"value": "kg", "lang": "en"}], "type": "unit group data set", "refObjectId": "ad38d542-3fe9-439d-9b95-2f5f7752acaf", "uri": "../unitgroups/ad38d542-3fe9-439d-9b95-2f5f7752acaf.xml"}}, {"value": "0.01714859", "module": "A1-A3"}, {"value": "1.49E-06", "module": "A4"}, {"value": "5.26E-05", "module": "A5"}, {"value": "0.87", "module": "B6"}, {"value": "0", "module": "C1"}, {"value": "5.58E-07", "module": "C2"}, {"value": "2.48E-06", "module": "C3"}, {"value": "4.16E-06", "module": "C4"}, {"value": "-0.00151", "module": "D"}]}, "resolvedFlowVersion": "38.00.000", "flowProperties": [], "typeOfFlow": "Other flow", "classification": {"classHierarchy": "Quantities / Environmental quantities / EPD EN 15804 / LCI indicators", "name": "GaBiCategories"}}, {"dataSetInternalID": 14, "referenceToFlowDataSet": {"shortDescription": [{"value": "Components for re-use (CRU)", "lang": "en"}, {"value": "Komponenten für die Wiederverwendung (CRU)", "lang": "de"}], "type": "flow data set", "refObjectId": "a2b32f97-3fc7-4af2-b209-525bc6426f33", "uri": "../flows/a2b32f97-3fc7-4af2-b209-525bc6426f33.xml"}, "exchange direction": "OUTPUT", "other": {"anies": [{"name": "referenceToUnitGroupDataSet", "value": {"shortDescription": [{"value": "kg", "lang": "en"}], "type": "unit group data set", "refObjectId": "ad38d542-3fe9-439d-9b95-2f5f7752acaf", "uri": "../unitgroups/ad38d542-3fe9-439d-9b95-2f5f7752acaf.xml"}}, {"value": "0", "module": "A1-A3"}, {"value": "0", "module": "A4"}, {"value": "0", "module": "A5"}, {"value": "0", "module": "B6"}, {"value": "0", "module": "C1"}, {"value": "0", "module": "C2"}, {"value": "0", "module": "C3"}, {"value": "0", "module": "C4"}, {"value": "0", "module": "D"}]}, "resolvedFlowVersion": "38.00.000", "flowProperties": [], "typeOfFlow": "Other flow", "classification": {"classHierarchy": "Quantities / Environmental quantities / EPD EN 15804 / LCI indicators", "name": "GaBiCategories"}}, {"dataSetInternalID": 15, "referenceToFlowDataSet": {"shortDescription": [{"value": "Materials for recycling (MFR)", "lang": "en"}, {"value": "Stoffe zum Recycling (MFR)", "lang": "de"}], "type": "flow data set", "refObjectId": "d7fe48a5-4103-49c8-9aae-b0b5dfdbd6ae", "uri": "../flows/d7fe48a5-4103-49c8-9aae-b0b5dfdbd6ae.xml"}, "exchange direction": "OUTPUT", "other": {"anies": [{"name": "referenceToUnitGroupDataSet", "value": {"shortDescription": [{"value": "kg", "lang": "en"}], "type": "unit group data set", "refObjectId": "ad38d542-3fe9-439d-9b95-2f5f7752acaf", "uri": "../unitgroups/ad38d542-3fe9-439d-9b95-2f5f7752acaf.xml"}}, {"value": "0", "module": "A1-A3"}, {"value": "0", "module": "A4"}, {"value": "0", "module": "A5"}, {"value": "0", "module": "B6"}, {"value": "0", "module": "C1"}, {"value": "0", "module": "C2"}, {"value": "7.38", "module": "C3"}, {"value": "0", "module": "C4"}, {"value": "0", "module": "D"}]}, "resolvedFlowVersion": "38.00.000", "flowProperties": [], "typeOfFlow": "Other flow", "classification": {"classHierarchy": "Quantities / Environmental quantities / EPD EN 15804 / LCI indicators", "name": "GaBiCategories"}}, {"dataSetInternalID": 16, "referenceToFlowDataSet": {"shortDescription": [{"value": "Materials for energy recovery (MER)", "lang": "en"}, {"value": "Stoffe für die Energierückgewinnung (MER)", "lang": "de"}], "type": "flow data set", "refObjectId": "59a9181c-3aaf-46ee-8b13-2b3723b6e447", "uri": "../flows/59a9181c-3aaf-46ee-8b13-2b3723b6e447.xml"}, "exchange direction": "OUTPUT", "other": {"anies": [{"name": "referenceToUnitGroupDataSet", "value": {"shortDescription": [{"value": "kg", "lang": "en"}], "type": "unit group data set", "refObjectId": "ad38d542-3fe9-439d-9b95-2f5f7752acaf", "uri": "../unitgroups/ad38d542-3fe9-439d-9b95-2f5f7752acaf.xml"}}, {"value": "0", "module": "A1-A3"}, {"value": "0", "module": "A4"}, {"value": "0", "module": "A5"}, {"value": "0", "module": "B6"}, {"value": "0", "module": "C1"}, {"value": "0", "module": "C2"}, {"value": "0", "module": "C3"}, {"value": "0", "module": "C4"}, {"value": "0", "module": "D"}]}, "resolvedFlowVersion": "38.00.000", "flowProperties": [], "typeOfFlow": "Other flow", "classification": {"classHierarchy": "Quantities / Environmental quantities / EPD EN 15804 / LCI indicators", "name": "GaBiCategories"}}, {"dataSetInternalID": 17, "referenceToFlowDataSet": {"shortDescription": [{"value": "Exported electrical energy (EEE)", "lang": "en"}, {"value": "Exportierte elektrische Energie (EEE)", "lang": "de"}], "type": "flow data set", "refObjectId": "4da0c987-2b76-40d6-9e9e-82a017aaaf29", "uri": "../flows/4da0c987-2b76-40d6-9e9e-82a017aaaf29.xml"}, "exchange direction": "OUTPUT", "other": {"anies": [{"name": "referenceToUnitGroupDataSet", "value": {"shortDescription": [{"value": "MJ", "lang": "en"}], "type": "unit group data set", "refObjectId": "93a60a57-a3c8-11da-a746-0800200c9a66", "uri": "../unitgroups/93a60a57-a3c8-11da-a746-0800200c9a66.xml"}}, {"value": "0.858", "module": "A1-A3"}, {"value": "0", "module": "A4"}, {"value": "4.81", "module": "A5"}, {"value": "0", "module": "B6"}, {"value": "0", "module": "C1"}, {"value": "0", "module": "C2"}, {"value": "0", "module": "C3"}, {"value": "0", "module": "C4"}, {"value": "0", "module": "D"}]}, "resolvedFlowVersion": "38.00.000", "flowProperties": [], "typeOfFlow": "Other flow", "classification": {"classHierarchy": "Quantities / Environmental quantities / EPD EN 15804 / LCI indicators", "name": "GaBiCategories"}}, {"dataSetInternalID": 18, "referenceToFlowDataSet": {"shortDescription": [{"value": "Exported thermal energy (EET)", "lang": "en"}, {"value": "Exportierte thermische Energie (EET)", "lang": "de"}], "type": "flow data set", "refObjectId": "98daf38a-7a79-46d3-9a37-2b7bd0955810", "uri": "../flows/98daf38a-7a79-46d3-9a37-2b7bd0955810.xml"}, "exchange direction": "OUTPUT", "other": {"anies": [{"name": "referenceToUnitGroupDataSet", "value": {"shortDescription": [{"value": "MJ", "lang": "en"}], "type": "unit group data set", "refObjectId": "93a60a57-a3c8-11da-a746-0800200c9a66", "uri": "../unitgroups/93a60a57-a3c8-11da-a746-0800200c9a66.xml"}}, {"value": "1.56", "module": "A1-A3"}, {"value": "0", "module": "A4"}, {"value": "8.77", "module": "A5"}, {"value": "0", "module": "B6"}, {"value": "0", "module": "C1"}, {"value": "0", "module": "C2"}, {"value": "0", "module": "C3"}, {"value": "0", "module": "C4"}, {"value": "0", "module": "D"}]}, "resolvedFlowVersion": "38.00.000", "flowProperties": [], "typeOfFlow": "Other flow", "classification": {"classHierarchy": "Quantities / Environmental quantities / EPD EN 15804 / LCI indicators", "name": "GaBiCategories"}}]}, "LCIAResults": {"LCIAResult": [{"referenceToLCIAMethodDataSet": {"shortDescription": [{"value": "Global Warming Potential total (GWP-total)", "lang": "en"}, {"value": "Globales Erwärmungspotenzial total (GWP-total)", "lang": "de"}], "type": "LCIA method data set", "refObjectId": "6a37f984-a4b3-458a-a20a-64418c145fa2", "uri": "../lciamethods/6a37f984-a4b3-458a-a20a-64418c145fa2.xml"}, "other": {"anies": [{"name": "referenceToUnitGroupDataSet", "value": {"shortDescription": [{"value": "kg CO_(2) eq", "lang": "en"}], "type": "unit group data set", "refObjectId": "1ebf3012-d0db-4de2-aefd-ef30cedb0be1", "uri": "../unitgroups/1ebf3012-d0db-4de2-aefd-ef30cedb0be1.xml"}}, {"value": "47.586", "module": "A1-A3"}, {"value": "0.102", "module": "A4"}, {"value": "3.17", "module": "A5"}, {"value": "328", "module": "B6"}, {"value": "0", "module": "C1"}, {"value": "0.0383", "module": "C2"}, {"value": "0.144", "module": "C3"}, {"value": "0.028", "module": "C4"}, {"value": "-2.31", "module": "D"}]}}, {"referenceToLCIAMethodDataSet": {"shortDescription": [{"value": "Global Warming Potential fossil fuels (GWP-fossil)", "lang": "en"}, {"value": "Globales Erwärmungspotenzial fossil (GWP-fossil)", "lang": "de"}], "type": "LCIA method data set", "refObjectId": "5f635281-343e-44fb-83df-1971b155e6b6", "uri": "../lciamethods/5f635281-343e-44fb-83df-1971b155e6b6.xml"}, "other": {"anies": [{"name": "referenceToUnitGroupDataSet", "value": {"shortDescription": [{"value": "kg CO_(2) eq", "lang": "en"}], "type": "unit group data set", "refObjectId": "1ebf3012-d0db-4de2-aefd-ef30cedb0be1", "uri": "../unitgroups/1ebf3012-d0db-4de2-aefd-ef30cedb0be1.xml"}}, {"value": "50.23", "module": "A1-A3"}, {"value": "0.0976", "module": "A4"}, {"value": "0.129", "module": "A5"}, {"value": "326", "module": "B6"}, {"value": "0", "module": "C1"}, {"value": "0.0366", "module": "C2"}, {"value": "0.144", "module": "C3"}, {"value": "0.0279", "module": "C4"}, {"value": "-2.31", "module": "D"}]}}, {"referenceToLCIAMethodDataSet": {"shortDescription": [{"value": "Global Warming Potential biogenic (GWP-biogenic)", "lang": "en"}, {"value": "Globales Erwärmungspotenzial biogen (GWP-biogenic)", "lang": "de"}], "type": "LCIA method data set", "refObjectId": "2356e1ab-0185-4db5-86e5-16de51c7485c", "uri": "../lciamethods/2356e1ab-0185-4db5-86e5-16de51c7485c.xml"}, "other": {"anies": [{"name": "referenceToUnitGroupDataSet", "value": {"shortDescription": [{"value": "kg CO_(2) eq", "lang": "en"}], "type": "unit group data set", "refObjectId": "1ebf3012-d0db-4de2-aefd-ef30cedb0be1", "uri": "../unitgroups/1ebf3012-d0db-4de2-aefd-ef30cedb0be1.xml"}}, {"value": "-2.72417", "module": "A1-A3"}, {"value": "0.00451", "module": "A4"}, {"value": "3.04", "module": "A5"}, {"value": "1.09", "module": "B6"}, {"value": "0", "module": "C1"}, {"value": "0.00169", "module": "C2"}, {"value": "3.35E-06", "module": "C3"}, {"value": "9.52E-05", "module": "C4"}, {"value": "0.00126", "module": "D"}]}}, {"referenceToLCIAMethodDataSet": {"shortDescription": [{"value": "Global Warming Potential luluc (GWP-luluc)", "lang": "en"}, {"value": "Globales Erwärmungspotenzial luluc (GWP-luluc)", "lang": "de"}], "type": "LCIA method data set", "refObjectId": "4331bbdb-978a-490d-8707-eeb047f01a55", "uri": "../lciamethods/4331bbdb-978a-490d-8707-eeb047f01a55.xml"}, "other": {"anies": [{"name": "referenceToUnitGroupDataSet", "value": {"shortDescription": [{"value": "kg CO_(2) eq", "lang": "en"}], "type": "unit group data set", "refObjectId": "1ebf3012-d0db-4de2-aefd-ef30cedb0be1", "uri": "../unitgroups/1ebf3012-d0db-4de2-aefd-ef30cedb0be1.xml"}}, {"value": "0.06997349", "module": "A1-A3"}, {"value": "2.32E-06", "module": "A4"}, {"value": "5.42E-05", "module": "A5"}, {"value": "0.473", "module": "B6"}, {"value": "0", "module": "C1"}, {"value": "8.72E-07", "module": "C2"}, {"value": "8.13E-06", "module": "C3"}, {"value": "8.02E-05", "module": "C4"}, {"value": "-0.00317", "module": "D"}]}}, {"referenceToLCIAMethodDataSet": {"shortDescription": [{"value": "Depletion potential of the stratospheric ozone layer (ODP)", "lang": "en"}, {"value": "Abbau Potential der stratosphärischen Ozonschicht (ODP)", "lang": "de"}], "type": "LCIA method data set", "refObjectId": "b5c629d6-def3-11e6-bf01-fe55135034f3", "uri": "../lciamethods/b5c629d6-def3-11e6-bf01-fe55135034f3.xml"}, "other": {"anies": [{"name": "referenceToUnitGroupDataSet", "value": {"shortDescription": [{"value": "kg CFC11 eq", "lang": "en"}], "type": "unit group data set", "refObjectId": "d9e957c9-7309-4474-bf3a-7777df6c4e5b", "uri": "../unitgroups/d9e957c9-7309-4474-bf3a-7777df6c4e5b.xml"}}, {"value": "3.490011111E-09", "module": "A1-A3"}, {"value": "1.03E-17", "module": "A4"}, {"value": "5.88E-16", "module": "A5"}, {"value": "7.18E-12", "module": "B6"}, {"value": "0", "module": "C1"}, {"value": "3.87E-18", "module": "C2"}, {"value": "7.26E-17", "module": "C3"}, {"value": "1.03E-16", "module": "C4"}, {"value": "-1.71E-14", "module": "D"}]}}, {"referenceToLCIAMethodDataSet": {"shortDescription": [{"value": "Acidification potential of land and water (AP)", "lang": "en"}, {"value": "Versauerungspotenzial von Boden und Wasser (AP)", "lang": "de"}], "type": "LCIA method data set", "refObjectId": "b5c611c6-def3-11e6-bf01-fe55135034f3", "uri": "../lciamethods/b5c611c6-def3-11e6-bf01-fe55135034f3.xml"}, "other": {"anies": [{"name": "referenceToUnitGroupDataSet", "value": {"shortDescription": [{"value": "mol H^(+) eq", "lang": "en"}], "type": "unit group data set", "refObjectId": "42e089ac-92bf-4bf2-8ca1-5fc40d18f2ed", "uri": "../unitgroups/42e089ac-92bf-4bf2-8ca1-5fc40d18f2ed.xml"}}, {"value": "0.299987", "module": "A1-A3"}, {"value": "9.77E-05", "module": "A4"}, {"value": "0.000883", "module": "A5"}, {"value": "0.72", "module": "B6"}, {"value": "0", "module": "C1"}, {"value": "3.67E-05", "module": "C2"}, {"value": "2.56E-05", "module": "C3"}, {"value": "0.0002", "module": "C4"}, {"value": "-0.0254", "module": "D"}]}}, {"referenceToLCIAMethodDataSet": {"shortDescription": [{"value": "Eutrophication potential aquatic freshwater (EP-freshwater)", "lang": "en"}, {"value": "Eutrophierungspotenzial Süßwasser (EP-freshwater)", "lang": "de"}], "type": "LCIA method data set", "refObjectId": "b53ec18f-7377-4ad3-86eb-cc3f4f276b2b", "uri": "../lciamethods/b53ec18f-7377-4ad3-86eb-cc3f4f276b2b.xml"}, "other": {"anies": [{"name": "referenceToUnitGroupDataSet", "value": {"shortDescription": [{"value": "kg P eq", "lang": "en"}], "type": "unit group data set", "refObjectId": "0429039d-a61d-4590-ba67-aa4a20a810a1", "uri": "../unitgroups/0429039d-a61d-4590-ba67-aa4a20a810a1.xml"}}, {"value": "0.0003378134", "module": "A1-A3"}, {"value": "2.09E-08", "module": "A4"}, {"value": "1.14E-07", "module": "A5"}, {"value": "0.000871", "module": "B6"}, {"value": "0", "module": "C1"}, {"value": "7.84E-09", "module": "C2"}, {"value": "1.16E-08", "module": "C3"}, {"value": "4.78E-08", "module": "C4"}, {"value": "-2.34E-06", "module": "D"}]}}, {"referenceToLCIAMethodDataSet": {"shortDescription": [{"value": "Eutrophication potential aquatic marine (EP-marine)", "lang": "en"}, {"value": "Eutrophierungspotenzial Salzwasser (EP-marine)", "lang": "de"}], "type": "LCIA method data set", "refObjectId": "b5c619fa-def3-11e6-bf01-fe55135034f3", "uri": "../lciamethods/b5c619fa-def3-11e6-bf01-fe55135034f3.xml"}, "other": {"anies": [{"name": "referenceToUnitGroupDataSet", "value": {"shortDescription": [{"value": "kg N eq", "lang": "en"}], "type": "unit group data set", "refObjectId": "d05bb823-ecdf-4686-8c40-bf1d9257859f", "uri": "../unitgroups/d05bb823-ecdf-4686-8c40-bf1d9257859f.xml"}}, {"value": "0.0455195", "module": "A1-A3"}, {"value": "3.11E-05", "module": "A4"}, {"value": "0.000317", "module": "A5"}, {"value": "0.16", "module": "B6"}, {"value": "0", "module": "C1"}, {"value": "1.17E-05", "module": "C2"}, {"value": "5.78E-06", "module": "C3"}, {"value": "5.14E-05", "module": "C4"}, {"value": "-0.00206", "module": "D"}]}}, {"referenceToLCIAMethodDataSet": {"shortDescription": [{"value": "Eutrophication potential terrestrial (EP-terrestrial)", "lang": "en"}, {"value": "Eutrophierungspotenzial Land (EP-terrestrial)", "lang": "de"}], "type": "LCIA method data set", "refObjectId": "b5c614d2-def3-11e6-bf01-fe55135034f3", "uri": "../lciamethods/b5c614d2-def3-11e6-bf01-fe55135034f3.xml"}, "other": {"anies": [{"name": "referenceToUnitGroupDataSet", "value": {"shortDescription": [{"value": "mol N eq", "lang": "en"}], "type": "unit group data set", "refObjectId": "71b4d617-0ec9-4d3f-b65e-e438940c2401", "uri": "../unitgroups/71b4d617-0ec9-4d3f-b65e-e438940c2401.xml"}}, {"value": "0.4823242", "module": "A1-A3"}, {"value": "0.000346", "module": "A4"}, {"value": "0.00397", "module": "A5"}, {"value": "1.68", "module": "B6"}, {"value": "0", "module": "C1"}, {"value": "0.00013", "module": "C2"}, {"value": "0.000117", "module": "C3"}, {"value": "0.000565", "module": "C4"}, {"value": "-0.0222", "module": "D"}]}}, {"referenceToLCIAMethodDataSet": {"shortDescription": [{"value": "Formation potential of tropospheric ozone photochemical oxidants (POCP)", "lang": "en"}, {"value": "Bildungspotential für troposphärisches Ozon (POCP)", "lang": "de"}], "type": "LCIA method data set", "refObjectId": "b5c610fe-def3-11e6-bf01-fe55135034f3", "uri": "../lciamethods/b5c610fe-def3-11e6-bf01-fe55135034f3.xml"}, "other": {"anies": [{"name": "referenceToUnitGroupDataSet", "value": {"shortDescription": [{"value": "kg NMVOC eq", "lang": "en"}], "type": "unit group data set", "refObjectId": "d27c25f8-fbc1-44c6-b47b-4adbae4199c6", "uri": "../unitgroups/d27c25f8-fbc1-44c6-b47b-4adbae4199c6.xml"}}, {"value": "0.1370416", "module": "A1-A3"}, {"value": "8.79E-05", "module": "A4"}, {"value": "0.000842", "module": "A5"}, {"value": "0.438", "module": "B6"}, {"value": "0", "module": "C1"}, {"value": "3.3E-05", "module": "C2"}, {"value": "1.6E-05", "module": "C3"}, {"value": "0.000156", "module": "C4"}, {"value": "-0.00672", "module": "D"}]}}, {"referenceToLCIAMethodDataSet": {"shortDescription": [{"value": "Abiotic depletion potential for non fossil resources (ADPE)", "lang": "en"}, {"value": "Potenzial für den abiotischen Abbau nicht fossiler Ressourcen (ADPE)", "lang": "de"}], "type": "LCIA method data set", "refObjectId": "b2ad6494-c78d-11e6-9d9d-cec0c932ce01", "uri": "../lciamethods/b2ad6494-c78d-11e6-9d9d-cec0c932ce01.xml"}, "other": {"anies": [{"name": "referenceToUnitGroupDataSet", "value": {"shortDescription": [{"value": "kg Sb eq", "lang": "en"}], "type": "unit group data set", "refObjectId": "54ccd2d9-a32a-4fc2-923d-f2c8c93e89d4", "uri": "../unitgroups/54ccd2d9-a32a-4fc2-923d-f2c8c93e89d4.xml"}}, {"value": "0.01060002103", "module": "A1-A3"}, {"value": "2.93E-09", "module": "A4"}, {"value": "9.23E-09", "module": "A5"}, {"value": "9.44E-05", "module": "B6"}, {"value": "0", "module": "C1"}, {"value": "1.1E-09", "module": "C2"}, {"value": "9.95E-10", "module": "C3"}, {"value": "2.5E-09", "module": "C4"}, {"value": "-0.00113", "module": "D"}]}}, {"referenceToLCIAMethodDataSet": {"shortDescription": [{"value": "Abiotic depletion potential for fossil resources (ADPF)", "lang": "en"}, {"value": "Potenzial für den abiotischen Abbau fossiler Brennstoffe (ADPF)", "lang": "de"}], "type": "LCIA method data set", "refObjectId": "b2ad6110-c78d-11e6-9d9d-cec0c932ce01", "uri": "../lciamethods/b2ad6110-c78d-11e6-9d9d-cec0c932ce01.xml"}, "other": {"anies": [{"name": "referenceToUnitGroupDataSet", "value": {"shortDescription": [{"value": "MJ", "lang": "en"}], "type": "unit group data set", "refObjectId": "93a60a57-a3c8-11da-a746-0800200c9a66", "uri": "../unitgroups/93a60a57-a3c8-11da-a746-0800200c9a66.xml"}}, {"value": "611.22", "module": "A1-A3"}, {"value": "1.38", "module": "A4"}, {"value": "1.01", "module": "A5"}, {"value": "5730", "module": "B6"}, {"value": "0", "module": "C1"}, {"value": "0.52", "module": "C2"}, {"value": "0.0667", "module": "C3"}, {"value": "0.366", "module": "C4"}, {"value": "-33.7", "module": "D"}]}}, {"referenceToLCIAMethodDataSet": {"shortDescription": [{"value": "Water use (WDP)", "lang": "en"}, {"value": "Wassernutzung (WDP)", "lang": "de"}], "type": "LCIA method data set", "refObjectId": "b2ad66ce-c78d-11e6-9d9d-cec0c932ce01", "uri": "../lciamethods/b2ad66ce-c78d-11e6-9d9d-cec0c932ce01.xml"}, "other": {"anies": [{"name": "referenceToUnitGroupDataSet", "value": {"shortDescription": [{"value": "m^(3) world eq deprived", "lang": "en"}], "type": "unit group data set", "refObjectId": "6ae2df01-888e-46c8-b17d-49fa3869b476", "uri": "../unitgroups/6ae2df01-888e-46c8-b17d-49fa3869b476.xml"}}, {"value": "13.483305", "module": "A1-A3"}, {"value": "0.000191", "module": "A4"}, {"value": "0.392", "module": "A5"}, {"value": "71.1", "module": "B6"}, {"value": "0", "module": "C1"}, {"value": "7.18E-05", "module": "C2"}, {"value": "0.0147", "module": "C3"}, {"value": "0.00292", "module": "C4"}, {"value": "-0.774", "module": "D"}]}}, {"referenceToLCIAMethodDataSet": {"shortDescription": [{"value": "Incidence of disease due to PM emissions (PM)", "lang": "en"}, {"value": "Auftreten von Krankheiten aufgrund von Feinstaubemissionen (PM)", "lang": "de"}], "type": "LCIA method data set", "refObjectId": "b5c602c6-def3-11e6-bf01-fe55135034f3", "uri": "../lciamethods/b5c602c6-def3-11e6-bf01-fe55135034f3.xml"}, "other": {"anies": [{"name": "referenceToUnitGroupDataSet", "value": {"shortDescription": [{"value": "Disease incidence", "lang": "en"}], "type": "unit group data set", "refObjectId": "3883559b-648f-4afc-8ba2-0bd24f3affa3", "uri": "../unitgroups/3883559b-648f-4afc-8ba2-0bd24f3affa3.xml"}}, {"value": "3.069139E-06", "module": "A1-A3"}, {"value": "5.14E-10", "module": "A4"}, {"value": "4.95E-09", "module": "A5"}, {"value": "6.04E-06", "module": "B6"}, {"value": "0", "module": "C1"}, {"value": "1.93E-10", "module": "C2"}, {"value": "3.27E-10", "module": "C3"}, {"value": "2.47E-09", "module": "C4"}, {"value": "-2.05E-07", "module": "D"}]}}, {"referenceToLCIAMethodDataSet": {"shortDescription": [{"value": "Human exposure efficiency relative to U235 (IR)", "lang": "en"}, {"value": "Wirkung durch Exposition des Menschen mit U235 (IR)", "lang": "de"}], "type": "LCIA method data set", "refObjectId": "b5c632be-def3-11e6-bf01-fe55135034f3", "uri": "../lciamethods/b5c632be-def3-11e6-bf01-fe55135034f3.xml"}, "other": {"anies": [{"name": "referenceToUnitGroupDataSet", "value": {"shortDescription": [{"value": "kBq U235 eq", "lang": "en"}], "type": "unit group data set", "refObjectId": "456b05bf-1415-44a9-9993-02452f554c09", "uri": "../unitgroups/456b05bf-1415-44a9-9993-02452f554c09.xml"}}, {"value": "1.688527", "module": "A1-A3"}, {"value": "0.000213", "module": "A4"}, {"value": "0.00809", "module": "A5"}, {"value": "143", "module": "B6"}, {"value": "0", "module": "C1"}, {"value": "7.98E-05", "module": "C2"}, {"value": "0.000223", "module": "C3"}, {"value": "0.000428", "module": "C4"}, {"value": "-0.244", "module": "D"}]}}, {"referenceToLCIAMethodDataSet": {"shortDescription": [{"value": "Comparative toxic unit for ecosystems (ETP-fw)", "lang": "en"}, {"value": "Toxizitätsvergleichseinheit für Ökosysteme (ETP-fw)", "lang": "de"}], "type": "LCIA method data set", "refObjectId": "ee1082d1-b0f7-43ca-a1f0-21e2a4a74511", "uri": "../lciamethods/ee1082d1-b0f7-43ca-a1f0-21e2a4a74511.xml"}, "other": {"anies": [{"name": "referenceToUnitGroupDataSet", "value": {"shortDescription": [{"value": "CTUe", "lang": "en"}], "type": "unit group data set", "refObjectId": "aa959ded-f1eb-4efb-9c5c-2d60be36b3e6", "uri": "../unitgroups/aa959ded-f1eb-4efb-9c5c-2d60be36b3e6.xml"}}, {"value": "296.426", "module": "A1-A3"}, {"value": "0.981", "module": "A4"}, {"value": "0.476", "module": "A5"}, {"value": "2450", "module": "B6"}, {"value": "0", "module": "C1"}, {"value": "0.368", "module": "C2"}, {"value": "0.025", "module": "C3"}, {"value": "0.209", "module": "C4"}, {"value": "-14.9", "module": "D"}]}}, {"referenceToLCIAMethodDataSet": {"shortDescription": [{"value": "Comparative toxic unit for humans (carcinogenic) (HTP-c)", "lang": "en"}, {"value": "Toxizitätsvergleichseinheit für Menschen (krebserregend) (HTP-c)", "lang": "de"}], "type": "LCIA method data set", "refObjectId": "2299222a-bbd8-474f-9d4f-4dd1f18aea7c", "uri": "../lciamethods/2299222a-bbd8-474f-9d4f-4dd1f18aea7c.xml"}, "other": {"anies": [{"name": "referenceToUnitGroupDataSet", "value": {"shortDescription": [{"value": "CTUh", "lang": "en"}], "type": "unit group data set", "refObjectId": "d4c9523e-2d7e-49fd-8469-998f547d3a70", "uri": "../unitgroups/d4c9523e-2d7e-49fd-8469-998f547d3a70.xml"}}, {"value": "4.17367E-08", "module": "A1-A3"}, {"value": "1.85E-11", "module": "A4"}, {"value": "2.55E-11", "module": "A5"}, {"value": "6.78E-08", "module": "B6"}, {"value": "0", "module": "C1"}, {"value": "6.93E-12", "module": "C2"}, {"value": "2.17E-12", "module": "C3"}, {"value": "3.09E-11", "module": "C4"}, {"value": "-1.07E-09", "module": "D"}]}}, {"referenceToLCIAMethodDataSet": {"shortDescription": [{"value": "Comparative toxic unit for humans (noncarcinogenic) (HTP-nc)", "lang": "en"}, {"value": "Toxizitätsvergleichseinheit für Menschen (nicht krebserregend) (HTP-nc)", "lang": "de"}], "type": "LCIA method data set", "refObjectId": "3af763a5-b7a1-48c9-9cee-1f223481fcef", "uri": "../lciamethods/3af763a5-b7a1-48c9-9cee-1f223481fcef.xml"}, "other": {"anies": [{"name": "referenceToUnitGroupDataSet", "value": {"shortDescription": [{"value": "CTUh", "lang": "en"}], "type": "unit group data set", "refObjectId": "d4c9523e-2d7e-49fd-8469-998f547d3a70", "uri": "../unitgroups/d4c9523e-2d7e-49fd-8469-998f547d3a70.xml"}}, {"value": "1.07996E-06", "module": "A1-A3"}, {"value": "7.89E-10", "module": "A4"}, {"value": "1.15E-09", "module": "A5"}, {"value": "2.5E-06", "module": "B6"}, {"value": "0", "module": "C1"}, {"value": "2.96E-10", "module": "C2"}, {"value": "2.19E-10", "module": "C3"}, {"value": "3.41E-09", "module": "C4"}, {"value": "-7.13E-08", "module": "D"}]}}, {"referenceToLCIAMethodDataSet": {"shortDescription": [{"value": "Soil quality index (SQP)", "lang": "en"}, {"value": "Bodenqualitätsindex (SQP)", "lang": "de"}], "type": "LCIA method data set", "refObjectId": "b2ad6890-c78d-11e6-9d9d-cec0c932ce01", "uri": "../lciamethods/b2ad6890-c78d-11e6-9d9d-cec0c932ce01.xml"}, "other": {"anies": [{"name": "referenceToUnitGroupDataSet", "value": {"shortDescription": [{"value": "SQP", "lang": "en"}], "type": "unit group data set", "refObjectId": "f130951c-e67f-4f7f-8dd4-665de3974e18", "uri": "../unitgroups/f130951c-e67f-4f7f-8dd4-665de3974e18.xml"}}, {"value": "543.73981", "module": "A1-A3"}, {"value": "0.00356", "module": "A4"}, {"value": "0.268", "module": "A5"}, {"value": "1830", "module": "B6"}, {"value": "0", "module": "C1"}, {"value": "0.00134", "module": "C2"}, {"value": "0.02", "module": "C3"}, {"value": "0.0762", "module": "C4"}, {"value": "-13.4", "module": "D"}]}}]}, "otherAttributes": {"{http://www.indata.network/EPD/2019}epd-version": "1.2"}, "version": "1.1", "locations": "../ILCDLocations.xml"}