{"processInformation": {"dataSetInformation": {"UUID": "2a7b2942-ff5d-4dca-8365-d4ffc28d013d", "name": {"baseName": [{"value": "Kooltherm® K15 C", "lang": "en"}], "functionalUnitFlowProperties": [{"lang": "en"}]}, "classificationInformation": {"classification": [{"class": [{"value": "Dämmstoffe", "level": 0, "classId": "2"}, {"value": "Phenolharz-Hartschaum (PF)", "level": 1, "classId": "2.5"}, {"value": "PF-Platten", "level": 2, "classId": "2.5.01"}], "name": "OEKOBAU.DAT"}, {"class": [{"value": "02 Building products", "level": 0}, {"value": "Thermal insulation products", "level": 1}, {"value": "Insulating materials made of foam plastics", "level": 2}], "name": "IBUCategories"}]}, "generalComment": [{"value": "The Kooltherm® K15 C is a rigid thermoset cellular insulation material faced on one side with microperforated aliminum based facing, and on other side with a mineral based glass tisue. The product is available in variable thicknesses from 20 mm up to 200 mm. This EPD covers one of the most commonly sold thickness of 100 mm with an RD-value of 5,0 m² K/W.", "lang": "en"}]}, "quantitativeReference": {"referenceToReferenceFlow": [0]}, "time": {"referenceYear": 2021, "dataSetValidUntil": 2026, "other": {"anies": [{"name": "publicationDateOfEPD", "value": 1616544000000}]}}, "geography": {"locationOfOperationSupplyOrProduction": {"location": "RER"}}, "technology": {"technologyDescriptionAndIncludedProcesses": [{"value": "Phenolic foam is produced by the use of phenolic resin, a catalyst, additives and blowing agent. The cell structure is formed in the resin under the influence of heat released during the chemical reaction. Hereby, the blowing agent is incorporated into the material which forms a solid and very fine cell structure, which is nearly 100% closed. The foam is applied on the facings. After this, the thickness and strength is determined by the conveyor belt where upper and lower rollers compress the material into the desired thickness. The board is sawed into the correct size and packed according to the product specification. \nDeclared unit: \nThe declared unit (1 m²) and conversion factors are\n\nlisted in the table below.", "lang": "en"}], "technologicalApplicability": [{"value": "Due to its high insulating value the Kooltherm® K15 C is suitable for use as insulation for ventilated facades in both new and renovation construction and also on concrete element in semi-sandwich constructions.", "lang": "en"}]}}, "modellingAndValidation": {"LCIMethodAndAllocation": {"typeOfDataSet": "EPD", "referenceToLCAMethodDetails": [{"shortDescription": [{"value": "Insulating materials made of foam plastics.pdf", "lang": "en"}], "type": "source data set", "refObjectId": "4ee3f11c-3093-4385-8cfa-0199635b12eb"}], "other": {"anies": [{"name": "subType", "value": "specific dataset"}]}}, "dataSourcesTreatmentAndRepresentativeness": {"referenceToDataSource": [{"shortDescription": [{"value": "GaBi Database (all versions)", "lang": "en"}], "type": "source data set", "refObjectId": "28d74cc0-db8b-4d7e-bc44-5f6d56ce0c4a"}, {"shortDescription": [{"value": "GaBi database SP39 2019", "lang": "en"}], "type": "source data set", "refObjectId": "07d9b8a7-e0fc-408f-a95e-c90735f843ce"}], "useAdviceForDataSet": [{"value": "Scope: \nThe insulation material Kooltherm® is produced by Kingspan Insulation B.V. at the manufacturing facility in Tiel, the Netherlands. A glass tissue based facing is autohesively bonded to the insulation core during manufacture. \n\nIn order to enable the user of the EPD to calculate the LCA results for different thicknesses, the EPD contains the respective calculation rules. \nSystem boundary: \nType of EPD: according to EN 15804: cradle to gate with options, modules C1–C4, and module D (A1–A3, C, D and additional modules: A4,A5).\n\nAccording to PCR Part A: \n\n1a) declaration of one specific product from one plant of one manufacturer.\n\nThe product stage is a mandatory information module and it covers:\n\n- A1, raw material extraction and processing, processing of secondary material input (e.g. recycling processes)\n\n- A2, transport to the manufacturer\n\n- A3, manufacturing,\n\nincluding the provision of all materials, products and energy, packaging processing and its transport, as well as waste processing up to the end-of waste state or disposal of final residues during the product stage.\n\nThe construction process stage includes:\n\n- A4 transport to the building site;\n\n- A5 installation in the building including provision of all materials, products and energy, as well as waste processing up to the end-of-waste state or disposal of final residues during the construction process stage. \n\n\nThe end-of-life stage is a mandatory information\n\nmodule and it covers:\n\n- C1 de-construction, demolition;\n\n- C2 transport to waste processing;\n\n- C3 waste processing for reuse, recovery and/or\n\nrecycling;\n\n- C4 disposal (not applicable for this EPD)\n\nincluding provision and all transport, provision of all\n\nmaterials, products and related energy and water use.\n\n\n\nEnvironmental burden of the incineration (R1 > 60%) of the product\n\nat the end-of-life stage are assigned to the product system (C3); resulting potential credits for thermal and electrical energy from energy substitution are declared in module D.\n\nRenewable electricity sources for manufacturing\n\n\nAll electricity used during production comes from\n\nrenewable sources. \n\nBy generating energy on-site with solar panels and with procured energy from fully certified renewable sources. Following the global Net Zero Energy strategy from Kingspan Group plc.", "lang": "en"}], "other": {"anies": [{"name": "referenceToOriginalEPD", "value": {"shortDescription": {"value": "Kooltherm® K15 C.pdf", "defaultValue": "Kooltherm® K15 C.pdf", "lstrings": [{"lang": "en", "value": "Kooltherm® K15 C.pdf"}]}, "type": "source data set", "uuid": {"uuid": "93074718-ff7a-4585-bf59-a163e30870de"}, "refObjectId": "93074718-ff7a-4585-bf59-a163e30870de", "resourceURLs": ["https://oekobaudat.de/OEKOBAU.DAT/resource/sources/93074718-ff7a-4585-bf59-a163e30870de/Kooltherm_K15_C_13195.pdf?version=00.01.000"]}}]}}, "validation": {"review": [{"referenceToNameOfReviewerAndInstitution": [{"shortDescription": [{"value": "Institut Bauen und Umwelt e. V.", "lang": "en"}], "type": "contact data set", "refObjectId": "d111dbec-b024-4be5-86c5-752d6eb2cf95", "uri": "../contacts/d111dbec-b024-4be5-86c5-752d6eb2cf95.xml"}], "type": "Accredited third party review"}]}, "complianceDeclarations": {"compliance": [{"referenceToComplianceSystem": {"shortDescription": [{"value": "DIN EN 15804+A2", "lang": "en"}], "type": "source data set", "refObjectId": "c0016b33-8cf7-415c-ac6e-deba0d21440d", "uri": "../sources/c0016b33-8cf7-415c-ac6e-deba0d21440d.xml"}}, {"referenceToComplianceSystem": {"shortDescription": [{"value": "ISO 14025", "lang": "en"}], "type": "source data set", "refObjectId": "4f2eb655-6e44-4874-a95a-e28f5442cd4d", "uri": "../sources/4f2eb655-6e44-4874-a95a-e28f5442cd4d.xml"}}]}}, "administrativeInformation": {"commissionerAndGoal": {"referenceToCommissioner": [{"shortDescription": [{"value": "Kingspan Insulation", "lang": "en"}], "type": "contact data set", "refObjectId": "bdf16a2b-22c1-4001-808e-1b515e7d0d56", "uri": "../contacts/bdf16a2b-22c1-4001-808e-1b515e7d0d56.xml"}]}, "dataGenerator": {"referenceToPersonOrEntityGeneratingTheDataSet": [{"shortDescription": [{"value": "Kingspan Insulation", "lang": "en"}], "type": "contact data set", "refObjectId": "bdf16a2b-22c1-4001-808e-1b515e7d0d56", "uri": "../contacts/bdf16a2b-22c1-4001-808e-1b515e7d0d56.xml"}]}, "dataEntryBy": {"timeStamp": 1616606297625, "referenceToDataSetFormat": [{"shortDescription": [{"value": "ILCD Format", "lang": "en"}], "type": "source data set", "refObjectId": "a97a0155-0234-4b87-b4ce-a45da52f2a40", "uri": "../sources/a97a0155-0234-4b87-b4ce-a45da52f2a40.xml"}, {"shortDescription": [{"value": "EPD-Datenformaterweiterungen v1.2", "lang": "de"}, {"value": "EPD Data Format Extensions v1.2", "lang": "en"}], "type": "source data set", "refObjectId": "a29449fd-aa2f-4de8-b5d7-4b06b43c6fde", "uri": "../sources/a29449fd-aa2f-4de8-b5d7-4b06b43c6fde.xml"}]}, "publicationAndOwnership": {"dataSetVersion": "00.02.000", "referenceToRegistrationAuthority": {"shortDescription": [{"value": "Institut Bauen und Umwelt e. V.", "lang": "en"}], "type": "contact data set", "refObjectId": "d111dbec-b024-4be5-86c5-752d6eb2cf95", "uri": "../contacts/d111dbec-b024-4be5-86c5-752d6eb2cf95.xml"}, "registrationNumber": "EPD-KSI-20200303-CBA1-EN", "referenceToOwnershipOfDataSet": {"shortDescription": [{"value": "Kingspan Insulation", "lang": "en"}], "type": "contact data set", "refObjectId": "bdf16a2b-22c1-4001-808e-1b515e7d0d56", "uri": "../contacts/bdf16a2b-22c1-4001-808e-1b515e7d0d56.xml"}, "copyright": true, "licenseType": "Free of charge for all users and uses", "accessRestrictions": [{"value": "None", "lang": "en"}], "other": {"anies": [{"name": "referenceToPublisher", "value": {"shortDescription": [{"value": "Institut Bauen und Umwelt e. V.", "lang": "en"}], "type": "contact data set", "refObjectId": "d111dbec-b024-4be5-86c5-752d6eb2cf95", "uri": "../contacts/d111dbec-b024-4be5-86c5-752d6eb2cf95.xml"}}]}}}, "exchanges": {"exchange": [{"dataSetInternalID": 0, "referenceToFlowDataSet": {"shortDescription": [{"value": "100 mm thickness (100 mm thickness)", "lang": "en"}], "type": "flow data set", "refObjectId": "fbffc0d9-e29a-ca3b-1453-fb3d9e7f75c4", "uri": "../flows/fbffc0d9-e29a-ca3b-1453-fb3d9e7f75c4.xml"}, "meanAmount": 1.0, "referencesToDataSource": {}, "referenceFlow": true, "resolvedFlowVersion": "00.02.000", "resultingflowAmount": 1.0, "flowProperties": [{"name": [{"lang": "en", "value": "Area"}, {"lang": "de", "value": "Fläche"}], "uuid": "93a60a56-a3c8-19da-a746-0800200c9a66", "referenceFlowProperty": true, "meanValue": 1.0, "referenceUnit": "qm", "unitGroupUUID": "c20a03d7-bd90-4569-bc94-66cfd364dfc8"}], "materialProperties": [{"name": "gross density", "value": "35.0", "unit": "kg/m^3", "unitDescription": "kilograms per cubic metre"}, {"name": "grammage", "value": "3.5", "unit": "kg/m^2", "unitDescription": "kilograms per square meter"}, {"name": "layer thickness", "value": "0.1", "unit": "m", "unitDescription": "meters"}, {"name": "conversion factor [mass/declared unit]", "value": "3.5", "unit": "-", "unitDescription": "Without unit"}], "typeOfFlow": "Product flow", "classification": {"classHierarchy": "Dämmstoffe / Phenolharz-Hartschaum (PF) / PF-Platten", "name": "OEKOBAU.DAT"}}, {"dataSetInternalID": 1, "referenceToFlowDataSet": {"shortDescription": [{"value": "Renewable primary energy as energy carrier (PERE)", "lang": "en"}], "type": "flow data set", "refObjectId": "20f32be5-0398-4288-9b6d-accddd195317", "uri": "../flows/20f32be5-0398-4288-9b6d-accddd195317.xml"}, "exchange direction": "INPUT", "other": {"anies": [{"name": "referenceToUnitGroupDataSet", "value": {"shortDescription": [{"value": "MJ", "lang": "en"}], "type": "unit group data set", "refObjectId": "93a60a57-a3c8-11da-a746-0800200c9a66", "uri": "../unitgroups/93a60a57-a3c8-11da-a746-0800200c9a66.xml"}}, {"value": "33.6", "module": "A1-A3"}, {"value": "0.02274", "module": "A4"}, {"value": "0.01527", "module": "A5"}, {"value": "8.919E-05", "module": "C1"}, {"value": "0.01137", "module": "C2"}, {"value": "0.2777", "module": "C3"}, {"value": "0", "module": "C4"}, {"value": "-1166", "module": "D"}]}, "resolvedFlowVersion": "38.00.000", "flowProperties": [], "typeOfFlow": "Other flow", "classification": {"classHierarchy": "Quantities", "name": "GaBiCategories"}}, {"dataSetInternalID": 2, "referenceToFlowDataSet": {"shortDescription": [{"value": "Renewable primary energy resources as material utilization (PERM)", "lang": "en"}], "type": "flow data set", "refObjectId": "fb3ec0de-548d-4508-aea5-00b73bf6f702", "uri": "../flows/fb3ec0de-548d-4508-aea5-00b73bf6f702.xml"}, "exchange direction": "INPUT", "other": {"anies": [{"name": "referenceToUnitGroupDataSet", "value": {"shortDescription": [{"value": "MJ", "lang": "en"}], "type": "unit group data set", "refObjectId": "93a60a57-a3c8-11da-a746-0800200c9a66", "uri": "../unitgroups/93a60a57-a3c8-11da-a746-0800200c9a66.xml"}}, {"value": "0", "module": "A1-A3"}, {"value": "0", "module": "A4"}, {"value": "0", "module": "A5"}, {"value": "0", "module": "C1"}, {"value": "0", "module": "C2"}, {"value": "0", "module": "C3"}, {"value": "0", "module": "C4"}, {"value": "0", "module": "D"}]}, "resolvedFlowVersion": "38.00.000", "flowProperties": [], "typeOfFlow": "Other flow", "classification": {"classHierarchy": "Quantities", "name": "GaBiCategories"}}, {"dataSetInternalID": 3, "referenceToFlowDataSet": {"shortDescription": [{"value": "Total use of renewable primary energy resources (PERT)", "lang": "en"}], "type": "flow data set", "refObjectId": "53f97275-fa8a-4cdd-9024-65936002acd0", "uri": "../flows/53f97275-fa8a-4cdd-9024-65936002acd0.xml"}, "exchange direction": "INPUT", "other": {"anies": [{"name": "referenceToUnitGroupDataSet", "value": {"shortDescription": [{"value": "MJ", "lang": "en"}], "type": "unit group data set", "refObjectId": "93a60a57-a3c8-11da-a746-0800200c9a66", "uri": "../unitgroups/93a60a57-a3c8-11da-a746-0800200c9a66.xml"}}, {"value": "33.6", "module": "A1-A3"}, {"value": "0.02274", "module": "A4"}, {"value": "0.01527", "module": "A5"}, {"value": "8.919E-05", "module": "C1"}, {"value": "0.01137", "module": "C2"}, {"value": "0.2777", "module": "C3"}, {"value": "0", "module": "C4"}, {"value": "-1166", "module": "D"}]}, "resolvedFlowVersion": "38.00.000", "flowProperties": [], "typeOfFlow": "Other flow", "classification": {"classHierarchy": "Quantities / Environmental quantities / EPD EN 15804 / LCI indicators", "name": "GaBiCategories"}}, {"dataSetInternalID": 4, "referenceToFlowDataSet": {"shortDescription": [{"value": "Non renewable primary energy as energy carrier (PENRE)", "lang": "en"}], "type": "flow data set", "refObjectId": "ac857178-2b45-46ec-892a-a9a4332f0372", "uri": "../flows/ac857178-2b45-46ec-892a-a9a4332f0372.xml"}, "exchange direction": "INPUT", "other": {"anies": [{"name": "referenceToUnitGroupDataSet", "value": {"shortDescription": [{"value": "MJ", "lang": "en"}], "type": "unit group data set", "refObjectId": "93a60a57-a3c8-11da-a746-0800200c9a66", "uri": "../unitgroups/93a60a57-a3c8-11da-a746-0800200c9a66.xml"}}, {"value": "92.7", "module": "A1-A3"}, {"value": "0.3921", "module": "A4"}, {"value": "0.07916", "module": "A5"}, {"value": "0.03036", "module": "C1"}, {"value": "0.1961", "module": "C2"}, {"value": "97.8", "module": "C3"}, {"value": "0", "module": "C4"}, {"value": "-57.52", "module": "D"}]}, "resolvedFlowVersion": "38.00.000", "flowProperties": [], "typeOfFlow": "Other flow", "classification": {"classHierarchy": "Quantities", "name": "GaBiCategories"}}, {"dataSetInternalID": 5, "referenceToFlowDataSet": {"shortDescription": [{"value": "Non renewable primary energy as material utilization (PENRM)", "lang": "en"}], "type": "flow data set", "refObjectId": "1421caa0-679d-4bf4-b282-0eb850ccae27", "uri": "../flows/1421caa0-679d-4bf4-b282-0eb850ccae27.xml"}, "exchange direction": "INPUT", "other": {"anies": [{"name": "referenceToUnitGroupDataSet", "value": {"shortDescription": [{"value": "MJ", "lang": "en"}], "type": "unit group data set", "refObjectId": "93a60a57-a3c8-11da-a746-0800200c9a66", "uri": "../unitgroups/93a60a57-a3c8-11da-a746-0800200c9a66.xml"}}, {"value": "95.8", "module": "A1-A3"}, {"value": "0", "module": "A4"}, {"value": "0", "module": "A5"}, {"value": "0", "module": "C1"}, {"value": "0", "module": "C2"}, {"value": "-95.8", "module": "C3"}, {"value": "0", "module": "C4"}, {"value": "0", "module": "D"}]}, "resolvedFlowVersion": "38.00.000", "flowProperties": [], "typeOfFlow": "Other flow", "classification": {"classHierarchy": "Quantities", "name": "GaBiCategories"}}, {"dataSetInternalID": 6, "referenceToFlowDataSet": {"shortDescription": [{"value": "Total use of non renewable primary energy resources (PENRT)", "lang": "en"}], "type": "flow data set", "refObjectId": "06159210-646b-4c8d-8583-da9b3b95a6c1", "uri": "../flows/06159210-646b-4c8d-8583-da9b3b95a6c1.xml"}, "exchange direction": "INPUT", "other": {"anies": [{"name": "referenceToUnitGroupDataSet", "value": {"shortDescription": [{"value": "MJ", "lang": "en"}], "type": "unit group data set", "refObjectId": "93a60a57-a3c8-11da-a746-0800200c9a66", "uri": "../unitgroups/93a60a57-a3c8-11da-a746-0800200c9a66.xml"}}, {"value": "188", "module": "A1-A3"}, {"value": "0.3921", "module": "A4"}, {"value": "0.07916", "module": "A5"}, {"value": "0.03036", "module": "C1"}, {"value": "0.1961", "module": "C2"}, {"value": "2.088", "module": "C3"}, {"value": "0", "module": "C4"}, {"value": "-57.52", "module": "D"}]}, "resolvedFlowVersion": "38.00.000", "flowProperties": [], "typeOfFlow": "Other flow", "classification": {"classHierarchy": "Quantities / Environmental quantities / EPD EN 15804 / LCI indicators", "name": "GaBiCategories"}}, {"dataSetInternalID": 7, "referenceToFlowDataSet": {"shortDescription": [{"value": "Use of secondary material (SM)", "lang": "en"}], "type": "flow data set", "refObjectId": "c6a1f35f-2d09-4f54-8dfb-97e502e1ce92", "uri": "../flows/c6a1f35f-2d09-4f54-8dfb-97e502e1ce92.xml"}, "exchange direction": "INPUT", "other": {"anies": [{"name": "referenceToUnitGroupDataSet", "value": {"shortDescription": [{"value": "kg", "lang": "en"}], "type": "unit group data set", "refObjectId": "ad38d542-3fe9-439d-9b95-2f5f7752acaf", "uri": "../unitgroups/ad38d542-3fe9-439d-9b95-2f5f7752acaf.xml"}}, {"value": "0", "module": "A1-A3"}, {"value": "0", "module": "A4"}, {"value": "0", "module": "A5"}, {"value": "0", "module": "C1"}, {"value": "0", "module": "C2"}, {"value": "0", "module": "C3"}, {"value": "0", "module": "C4"}, {"value": "0", "module": "D"}]}, "resolvedFlowVersion": "38.00.000", "flowProperties": [], "typeOfFlow": "Other flow", "classification": {"classHierarchy": "Quantities / Environmental quantities / EPD EN 15804 / LCI indicators", "name": "GaBiCategories"}}, {"dataSetInternalID": 8, "referenceToFlowDataSet": {"shortDescription": [{"value": "Use of renewable secondary fuels (RSF)", "lang": "en"}], "type": "flow data set", "refObjectId": "64333088-a55f-4aa2-9a31-c10b07816787", "uri": "../flows/64333088-a55f-4aa2-9a31-c10b07816787.xml"}, "exchange direction": "INPUT", "other": {"anies": [{"name": "referenceToUnitGroupDataSet", "value": {"shortDescription": [{"value": "MJ", "lang": "en"}], "type": "unit group data set", "refObjectId": "93a60a57-a3c8-11da-a746-0800200c9a66", "uri": "../unitgroups/93a60a57-a3c8-11da-a746-0800200c9a66.xml"}}, {"value": "0", "module": "A1-A3"}, {"value": "0", "module": "A4"}, {"value": "0", "module": "A5"}, {"value": "0", "module": "C1"}, {"value": "0", "module": "C2"}, {"value": "0", "module": "C3"}, {"value": "0", "module": "C4"}, {"value": "0", "module": "D"}]}, "resolvedFlowVersion": "38.00.000", "flowProperties": [], "typeOfFlow": "Other flow", "classification": {"classHierarchy": "Quantities / Environmental quantities / EPD EN 15804 / LCI indicators", "name": "GaBiCategories"}}, {"dataSetInternalID": 9, "referenceToFlowDataSet": {"shortDescription": [{"value": "Use of non renewable secondary fuels (NRSF)", "lang": "en"}], "type": "flow data set", "refObjectId": "89def144-d39a-4287-b86f-efde453ddcb2", "uri": "../flows/89def144-d39a-4287-b86f-efde453ddcb2.xml"}, "exchange direction": "INPUT", "other": {"anies": [{"name": "referenceToUnitGroupDataSet", "value": {"shortDescription": [{"value": "MJ", "lang": "en"}], "type": "unit group data set", "refObjectId": "93a60a57-a3c8-11da-a746-0800200c9a66", "uri": "../unitgroups/93a60a57-a3c8-11da-a746-0800200c9a66.xml"}}, {"value": "0", "module": "A1-A3"}, {"value": "0", "module": "A4"}, {"value": "0", "module": "A5"}, {"value": "0", "module": "C1"}, {"value": "0", "module": "C2"}, {"value": "0", "module": "C3"}, {"value": "0", "module": "C4"}, {"value": "0", "module": "D"}]}, "resolvedFlowVersion": "38.00.000", "flowProperties": [], "typeOfFlow": "Other flow", "classification": {"classHierarchy": "Quantities / Environmental quantities / EPD EN 15804 / LCI indicators", "name": "GaBiCategories"}}, {"dataSetInternalID": 10, "referenceToFlowDataSet": {"shortDescription": [{"value": "Use of net fresh water (FW)", "lang": "en"}], "type": "flow data set", "refObjectId": "3cf952c8-f3a4-461d-8c96-96456ca62246", "uri": "../flows/3cf952c8-f3a4-461d-8c96-96456ca62246.xml"}, "exchange direction": "INPUT", "other": {"anies": [{"name": "referenceToUnitGroupDataSet", "value": {"shortDescription": [{"value": "m^3", "lang": "en"}], "type": "unit group data set", "refObjectId": "cd950537-0a98-4044-9ba7-9f9a68d0a504", "uri": "../unitgroups/cd950537-0a98-4044-9ba7-9f9a68d0a504.xml"}}, {"value": "0.058553", "module": "A1-A3"}, {"value": "3.845E-05", "module": "A4"}, {"value": "0.0004943", "module": "A5"}, {"value": "1.646E-07", "module": "C1"}, {"value": "1.923E-05", "module": "C2"}, {"value": "0.01789", "module": "C3"}, {"value": "0", "module": "C4"}, {"value": "-0.01374", "module": "D"}]}, "resolvedFlowVersion": "38.00.000", "flowProperties": [], "typeOfFlow": "Other flow", "classification": {"classHierarchy": "Quantities / Environmental quantities / EPD EN 15804 / LCI indicators", "name": "GaBiCategories"}}, {"dataSetInternalID": 11, "referenceToFlowDataSet": {"shortDescription": [{"value": "Hazardous waste disposed (HWD)", "lang": "en"}], "type": "flow data set", "refObjectId": "430f9e0f-59b2-46a0-8e0d-55e0e84948fc", "uri": "../flows/430f9e0f-59b2-46a0-8e0d-55e0e84948fc.xml"}, "exchange direction": "OUTPUT", "other": {"anies": [{"name": "referenceToUnitGroupDataSet", "value": {"shortDescription": [{"value": "kg", "lang": "en"}], "type": "unit group data set", "refObjectId": "ad38d542-3fe9-439d-9b95-2f5f7752acaf", "uri": "../unitgroups/ad38d542-3fe9-439d-9b95-2f5f7752acaf.xml"}}, {"value": "8.33E-05", "module": "A1-A3"}, {"value": "2.19E-08", "module": "A4"}, {"value": "3.707E-10", "module": "A5"}, {"value": "3.217E-12", "module": "C1"}, {"value": "1.095E-08", "module": "C2"}, {"value": "1.327E-09", "module": "C3"}, {"value": "0", "module": "C4"}, {"value": "-2.367E-08", "module": "D"}]}, "resolvedFlowVersion": "38.00.000", "flowProperties": [], "typeOfFlow": "Other flow", "classification": {"classHierarchy": "Quantities / Environmental quantities / EPD EN 15804 / LCI indicators", "name": "GaBiCategories"}}, {"dataSetInternalID": 12, "referenceToFlowDataSet": {"shortDescription": [{"value": "Non hazardous waste disposed (NHWD)", "lang": "en"}], "type": "flow data set", "refObjectId": "b29ef66b-e286-4afa-949f-62f1a7b4d7fa", "uri": "../flows/b29ef66b-e286-4afa-949f-62f1a7b4d7fa.xml"}, "exchange direction": "OUTPUT", "other": {"anies": [{"name": "referenceToUnitGroupDataSet", "value": {"shortDescription": [{"value": "kg", "lang": "en"}], "type": "unit group data set", "refObjectId": "ad38d542-3fe9-439d-9b95-2f5f7752acaf", "uri": "../unitgroups/ad38d542-3fe9-439d-9b95-2f5f7752acaf.xml"}}, {"value": "0.412", "module": "A1-A3"}, {"value": "3.187E-05", "module": "A4"}, {"value": "0.01931", "module": "A5"}, {"value": "1.812E-07", "module": "C1"}, {"value": "1.594E-05", "module": "C2"}, {"value": "0.03882", "module": "C3"}, {"value": "0", "module": "C4"}, {"value": "-0.02486", "module": "D"}]}, "resolvedFlowVersion": "38.00.000", "flowProperties": [], "typeOfFlow": "Other flow", "classification": {"classHierarchy": "Quantities / Environmental quantities / EPD EN 15804 / LCI indicators", "name": "GaBiCategories"}}, {"dataSetInternalID": 13, "referenceToFlowDataSet": {"shortDescription": [{"value": "Radioactive waste disposed (RWD)", "lang": "en"}], "type": "flow data set", "refObjectId": "3449546e-52ad-4b39-b809-9fb77cea8ff6", "uri": "../flows/3449546e-52ad-4b39-b809-9fb77cea8ff6.xml"}, "exchange direction": "OUTPUT", "other": {"anies": [{"name": "referenceToUnitGroupDataSet", "value": {"shortDescription": [{"value": "kg", "lang": "en"}], "type": "unit group data set", "refObjectId": "ad38d542-3fe9-439d-9b95-2f5f7752acaf", "uri": "../unitgroups/ad38d542-3fe9-439d-9b95-2f5f7752acaf.xml"}}, {"value": "0.00309", "module": "A1-A3"}, {"value": "5.32E-07", "module": "A4"}, {"value": "3.641E-06", "module": "A5"}, {"value": "3.492E-08", "module": "C1"}, {"value": "2.66E-07", "module": "C2"}, {"value": "9.391E-05", "module": "C3"}, {"value": "0", "module": "C4"}, {"value": "-0.004651", "module": "D"}]}, "resolvedFlowVersion": "38.00.000", "flowProperties": [], "typeOfFlow": "Other flow", "classification": {"classHierarchy": "Quantities / Environmental quantities / EPD EN 15804 / LCI indicators", "name": "GaBiCategories"}}, {"dataSetInternalID": 14, "referenceToFlowDataSet": {"shortDescription": [{"value": "Components for re-use (CRU)", "lang": "en"}], "type": "flow data set", "refObjectId": "a2b32f97-3fc7-4af2-b209-525bc6426f33", "uri": "../flows/a2b32f97-3fc7-4af2-b209-525bc6426f33.xml"}, "exchange direction": "OUTPUT", "other": {"anies": [{"name": "referenceToUnitGroupDataSet", "value": {"shortDescription": [{"value": "kg", "lang": "en"}], "type": "unit group data set", "refObjectId": "ad38d542-3fe9-439d-9b95-2f5f7752acaf", "uri": "../unitgroups/ad38d542-3fe9-439d-9b95-2f5f7752acaf.xml"}}, {"value": "0", "module": "A1-A3"}, {"value": "0", "module": "A4"}, {"value": "0", "module": "A5"}, {"value": "0", "module": "C1"}, {"value": "0", "module": "C2"}, {"value": "0", "module": "C3"}, {"value": "0", "module": "C4"}, {"value": "0", "module": "D"}]}, "resolvedFlowVersion": "38.00.000", "flowProperties": [], "typeOfFlow": "Other flow", "classification": {"classHierarchy": "Quantities / Environmental quantities / EPD EN 15804 / LCI indicators", "name": "GaBiCategories"}}, {"dataSetInternalID": 15, "referenceToFlowDataSet": {"shortDescription": [{"value": "Materials for recycling (MFR)", "lang": "en"}], "type": "flow data set", "refObjectId": "d7fe48a5-4103-49c8-9aae-b0b5dfdbd6ae", "uri": "../flows/d7fe48a5-4103-49c8-9aae-b0b5dfdbd6ae.xml"}, "exchange direction": "OUTPUT", "other": {"anies": [{"name": "referenceToUnitGroupDataSet", "value": {"shortDescription": [{"value": "kg", "lang": "en"}], "type": "unit group data set", "refObjectId": "ad38d542-3fe9-439d-9b95-2f5f7752acaf", "uri": "../unitgroups/ad38d542-3fe9-439d-9b95-2f5f7752acaf.xml"}}, {"value": "0", "module": "A1-A3"}, {"value": "0", "module": "A4"}, {"value": "0", "module": "A5"}, {"value": "0", "module": "C1"}, {"value": "0", "module": "C2"}, {"value": "0", "module": "C3"}, {"value": "0", "module": "C4"}, {"value": "0", "module": "D"}]}, "resolvedFlowVersion": "38.00.000", "flowProperties": [], "typeOfFlow": "Other flow", "classification": {"classHierarchy": "Quantities / Environmental quantities / EPD EN 15804 / LCI indicators", "name": "GaBiCategories"}}, {"dataSetInternalID": 16, "referenceToFlowDataSet": {"shortDescription": [{"value": "Materials for energy recovery (MER)", "lang": "en"}], "type": "flow data set", "refObjectId": "59a9181c-3aaf-46ee-8b13-2b3723b6e447", "uri": "../flows/59a9181c-3aaf-46ee-8b13-2b3723b6e447.xml"}, "exchange direction": "OUTPUT", "other": {"anies": [{"name": "referenceToUnitGroupDataSet", "value": {"shortDescription": [{"value": "kg", "lang": "en"}], "type": "unit group data set", "refObjectId": "ad38d542-3fe9-439d-9b95-2f5f7752acaf", "uri": "../unitgroups/ad38d542-3fe9-439d-9b95-2f5f7752acaf.xml"}}, {"value": "0", "module": "A1-A3"}, {"value": "0", "module": "A4"}, {"value": "0.0799", "module": "A5"}, {"value": "0", "module": "C1"}, {"value": "0", "module": "C2"}, {"value": "3.5", "module": "C3"}, {"value": "0", "module": "C4"}, {"value": "0", "module": "D"}]}, "resolvedFlowVersion": "38.00.000", "flowProperties": [], "typeOfFlow": "Other flow", "classification": {"classHierarchy": "Quantities / Environmental quantities / EPD EN 15804 / LCI indicators", "name": "GaBiCategories"}}, {"dataSetInternalID": 17, "referenceToFlowDataSet": {"shortDescription": [{"value": "Exported electrical energy (EEE)", "lang": "en"}], "type": "flow data set", "refObjectId": "4da0c987-2b76-40d6-9e9e-82a017aaaf29", "uri": "../flows/4da0c987-2b76-40d6-9e9e-82a017aaaf29.xml"}, "exchange direction": "OUTPUT", "other": {"anies": [{"name": "referenceToUnitGroupDataSet", "value": {"shortDescription": [{"value": "MJ", "lang": "en"}], "type": "unit group data set", "refObjectId": "93a60a57-a3c8-11da-a746-0800200c9a66", "uri": "../unitgroups/93a60a57-a3c8-11da-a746-0800200c9a66.xml"}}, {"value": "0", "module": "A1-A3"}, {"value": "0", "module": "A4"}, {"value": "0.4426", "module": "A5"}, {"value": "0", "module": "C1"}, {"value": "0", "module": "C2"}, {"value": "13.35", "module": "C3"}, {"value": "0", "module": "C4"}, {"value": "0", "module": "D"}]}, "resolvedFlowVersion": "38.00.000", "flowProperties": [], "typeOfFlow": "Other flow", "classification": {"classHierarchy": "Quantities / Environmental quantities / EPD EN 15804 / LCI indicators", "name": "GaBiCategories"}}, {"dataSetInternalID": 18, "referenceToFlowDataSet": {"shortDescription": [{"value": "Exported thermal energy (EET)", "lang": "en"}], "type": "flow data set", "refObjectId": "98daf38a-7a79-46d3-9a37-2b7bd0955810", "uri": "../flows/98daf38a-7a79-46d3-9a37-2b7bd0955810.xml"}, "exchange direction": "OUTPUT", "other": {"anies": [{"name": "referenceToUnitGroupDataSet", "value": {"shortDescription": [{"value": "MJ", "lang": "en"}], "type": "unit group data set", "refObjectId": "93a60a57-a3c8-11da-a746-0800200c9a66", "uri": "../unitgroups/93a60a57-a3c8-11da-a746-0800200c9a66.xml"}}, {"value": "0", "module": "A1-A3"}, {"value": "0", "module": "A4"}, {"value": "0.7979", "module": "A5"}, {"value": "0", "module": "C1"}, {"value": "0", "module": "C2"}, {"value": "23.88", "module": "C3"}, {"value": "0", "module": "C4"}, {"value": "0", "module": "D"}]}, "resolvedFlowVersion": "38.00.000", "flowProperties": [], "typeOfFlow": "Other flow", "classification": {"classHierarchy": "Quantities / Environmental quantities / EPD EN 15804 / LCI indicators", "name": "GaBiCategories"}}]}, "LCIAResults": {"LCIAResult": [{"referenceToLCIAMethodDataSet": {"shortDescription": [{"value": "Global Warming Potential total (GWP-total)", "lang": "en"}], "type": "LCIA method data set", "refObjectId": "6a37f984-a4b3-458a-a20a-64418c145fa2", "uri": "../lciamethods/6a37f984-a4b3-458a-a20a-64418c145fa2.xml"}, "other": {"anies": [{"name": "referenceToUnitGroupDataSet", "value": {"shortDescription": [{"value": "kg CO_(2)-Äq.", "lang": "en"}], "type": "unit group data set", "refObjectId": "1ebf3012-d0db-4de2-aefd-ef30cedb0be1", "uri": "../unitgroups/1ebf3012-d0db-4de2-aefd-ef30cedb0be1.xml"}}, {"value": "7.168", "module": "A1-A3"}, {"value": "0.02966", "module": "A4"}, {"value": "0.2", "module": "A5"}, {"value": "0.002238", "module": "C1"}, {"value": "0.01483", "module": "C2"}, {"value": "7.73", "module": "C3"}, {"value": "0", "module": "C4"}, {"value": "-3.32", "module": "D"}]}}, {"referenceToLCIAMethodDataSet": {"shortDescription": [{"value": "Global Warming Potential fossil fuels (GWP-fossil)", "lang": "en"}], "type": "LCIA method data set", "refObjectId": "5f635281-343e-44fb-83df-1971b155e6b6", "uri": "../lciamethods/5f635281-343e-44fb-83df-1971b155e6b6.xml"}, "other": {"anies": [{"name": "referenceToUnitGroupDataSet", "value": {"shortDescription": [{"value": "kg CO_(2)-Äq.", "lang": "en"}], "type": "unit group data set", "refObjectId": "1ebf3012-d0db-4de2-aefd-ef30cedb0be1", "uri": "../unitgroups/1ebf3012-d0db-4de2-aefd-ef30cedb0be1.xml"}}, {"value": "7.116", "module": "A1-A3"}, {"value": "0.02939", "module": "A4"}, {"value": "0.2", "module": "A5"}, {"value": "0.002238", "module": "C1"}, {"value": "0.0147", "module": "C2"}, {"value": "7.729", "module": "C3"}, {"value": "0", "module": "C4"}, {"value": "-3.32", "module": "D"}]}}, {"referenceToLCIAMethodDataSet": {"shortDescription": [{"value": "Global Warming Potential biogenic (GWP-biogenic)", "lang": "en"}], "type": "LCIA method data set", "refObjectId": "2356e1ab-0185-4db5-86e5-16de51c7485c", "uri": "../lciamethods/2356e1ab-0185-4db5-86e5-16de51c7485c.xml"}, "other": {"anies": [{"name": "referenceToUnitGroupDataSet", "value": {"shortDescription": [{"value": "kg CO_(2)-Äq.", "lang": "en"}], "type": "unit group data set", "refObjectId": "1ebf3012-d0db-4de2-aefd-ef30cedb0be1", "uri": "../unitgroups/1ebf3012-d0db-4de2-aefd-ef30cedb0be1.xml"}}, {"value": "-0.0194", "module": "A1-A3"}, {"value": "-0.0001788", "module": "A4"}, {"value": "-3.632E-06", "module": "A5"}, {"value": "-1.577E-07", "module": "C1"}, {"value": "-8.94E-05", "module": "C2"}, {"value": "0.0003465", "module": "C3"}, {"value": "0", "module": "C4"}, {"value": "-0.006444", "module": "D"}]}}, {"referenceToLCIAMethodDataSet": {"shortDescription": [{"value": "Global Warming Potential luluc (GWP-luluc)", "lang": "en"}], "type": "LCIA method data set", "refObjectId": "4331bbdb-978a-490d-8707-eeb047f01a55", "uri": "../lciamethods/4331bbdb-978a-490d-8707-eeb047f01a55.xml"}, "other": {"anies": [{"name": "referenceToUnitGroupDataSet", "value": {"shortDescription": [{"value": "kg CO_(2)-Äq.", "lang": "en"}], "type": "unit group data set", "refObjectId": "1ebf3012-d0db-4de2-aefd-ef30cedb0be1", "uri": "../unitgroups/1ebf3012-d0db-4de2-aefd-ef30cedb0be1.xml"}}, {"value": "0.072", "module": "A1-A3"}, {"value": "0.0004495", "module": "A4"}, {"value": "7.199E-06", "module": "A5"}, {"value": "7.594E-08", "module": "C1"}, {"value": "0.0002247", "module": "C2"}, {"value": "7.469E-05", "module": "C3"}, {"value": "0", "module": "C4"}, {"value": "-0.002264", "module": "D"}]}}, {"referenceToLCIAMethodDataSet": {"shortDescription": [{"value": "Depletion potential of the stratospheric ozone layer (ODP)", "lang": "en"}], "type": "LCIA method data set", "refObjectId": "b5c629d6-def3-11e6-bf01-fe55135034f3", "uri": "../lciamethods/b5c629d6-def3-11e6-bf01-fe55135034f3.xml"}, "other": {"anies": [{"name": "referenceToUnitGroupDataSet", "value": {"shortDescription": [{"value": "kg CFC11-Äq.", "lang": "en"}], "type": "unit group data set", "refObjectId": "d9e957c9-7309-4474-bf3a-7777df6c4e5b", "uri": "../unitgroups/d9e957c9-7309-4474-bf3a-7777df6c4e5b.xml"}}, {"value": "1.23E-08", "module": "A1-A3"}, {"value": "3.572E-18", "module": "A4"}, {"value": "5.97E-17", "module": "A5"}, {"value": "2.15E-19", "module": "C1"}, {"value": "1.786E-18", "module": "C2"}, {"value": "9.264E-16", "module": "C3"}, {"value": "0", "module": "C4"}, {"value": "-3.397E-14", "module": "D"}]}}, {"referenceToLCIAMethodDataSet": {"shortDescription": [{"value": "Acidification potential of land and water (AP)", "lang": "en"}], "type": "LCIA method data set", "refObjectId": "b5c611c6-def3-11e6-bf01-fe55135034f3", "uri": "../lciamethods/b5c611c6-def3-11e6-bf01-fe55135034f3.xml"}, "other": {"anies": [{"name": "referenceToUnitGroupDataSet", "value": {"shortDescription": [{"value": "mol H^(+)-Äq.", "lang": "en"}], "type": "unit group data set", "refObjectId": "42e089ac-92bf-4bf2-8ca1-5fc40d18f2ed", "uri": "../unitgroups/42e089ac-92bf-4bf2-8ca1-5fc40d18f2ed.xml"}}, {"value": "0.0214", "module": "A1-A3"}, {"value": "3.471E-05", "module": "A4"}, {"value": "2.757E-05", "module": "A5"}, {"value": "1.735E-05", "module": "C1"}, {"value": "1.735E-05", "module": "C2"}, {"value": "0.004615", "module": "C3"}, {"value": "0", "module": "C4"}, {"value": "-0.006279", "module": "D"}]}}, {"referenceToLCIAMethodDataSet": {"shortDescription": [{"value": "Eutrophication potential aquatic freshwater (EP-freshwater)", "lang": "en"}], "type": "LCIA method data set", "refObjectId": "b53ec18f-7377-4ad3-86eb-cc3f4f276b2b", "uri": "../lciamethods/b53ec18f-7377-4ad3-86eb-cc3f4f276b2b.xml"}, "other": {"anies": [{"name": "referenceToUnitGroupDataSet", "value": {"shortDescription": [{"value": "kg PO_(4)-Äq.", "lang": "en"}], "type": "unit group data set", "refObjectId": "0429039d-a61d-4590-ba67-aa4a20a810a1", "uri": "../unitgroups/0429039d-a61d-4590-ba67-aa4a20a810a1.xml"}}, {"value": "0.000188", "module": "A1-A3"}, {"value": "1.418E-07", "module": "A4"}, {"value": "1.053E-08", "module": "A5"}, {"value": "3.977E-10", "module": "C1"}, {"value": "7.091E-08", "module": "C2"}, {"value": "1.575E-07", "module": "C3"}, {"value": "0", "module": "C4"}, {"value": "-4.37E-06", "module": "D"}]}}, {"referenceToLCIAMethodDataSet": {"shortDescription": [{"value": "Eutrophication potential aquatic marine (EP-marine)", "lang": "en"}], "type": "LCIA method data set", "refObjectId": "b5c619fa-def3-11e6-bf01-fe55135034f3", "uri": "../lciamethods/b5c619fa-def3-11e6-bf01-fe55135034f3.xml"}, "other": {"anies": [{"name": "referenceToUnitGroupDataSet", "value": {"shortDescription": [{"value": "kg N-Äq.", "lang": "en"}], "type": "unit group data set", "refObjectId": "d05bb823-ecdf-4686-8c40-bf1d9257859f", "uri": "../unitgroups/d05bb823-ecdf-4686-8c40-bf1d9257859f.xml"}}, {"value": "0.004797", "module": "A1-A3"}, {"value": "1.07E-05", "module": "A4"}, {"value": "7.281E-06", "module": "A5"}, {"value": "4.968E-06", "module": "C1"}, {"value": "5.351E-06", "module": "C2"}, {"value": "0.002215", "module": "C3"}, {"value": "0", "module": "C4"}, {"value": "-0.001443", "module": "D"}]}}, {"referenceToLCIAMethodDataSet": {"shortDescription": [{"value": "Eutrophication potential terrestrial (EP-terrestrial)", "lang": "en"}], "type": "LCIA method data set", "refObjectId": "b5c614d2-def3-11e6-bf01-fe55135034f3", "uri": "../lciamethods/b5c614d2-def3-11e6-bf01-fe55135034f3.xml"}, "other": {"anies": [{"name": "referenceToUnitGroupDataSet", "value": {"shortDescription": [{"value": "mol N-Äq.", "lang": "en"}], "type": "unit group data set", "refObjectId": "71b4d617-0ec9-4d3f-b65e-e438940c2401", "uri": "../unitgroups/71b4d617-0ec9-4d3f-b65e-e438940c2401.xml"}}, {"value": "0.04891", "module": "A1-A3"}, {"value": "0.0001254", "module": "A4"}, {"value": "0.0001198", "module": "A5"}, {"value": "5.442E-05", "module": "C1"}, {"value": "6.268E-05", "module": "C2"}, {"value": "0.02548", "module": "C3"}, {"value": "0", "module": "C4"}, {"value": "-0.01548", "module": "D"}]}}, {"referenceToLCIAMethodDataSet": {"shortDescription": [{"value": "Formation potential of tropospheric ozone photochemical oxidants (POCP)", "lang": "en"}], "type": "LCIA method data set", "refObjectId": "b5c610fe-def3-11e6-bf01-fe55135034f3", "uri": "../lciamethods/b5c610fe-def3-11e6-bf01-fe55135034f3.xml"}, "other": {"anies": [{"name": "referenceToUnitGroupDataSet", "value": {"shortDescription": [{"value": "kg NMVOC-Äq.", "lang": "en"}], "type": "unit group data set", "refObjectId": "d27c25f8-fbc1-44c6-b47b-4adbae4199c6", "uri": "../unitgroups/d27c25f8-fbc1-44c6-b47b-4adbae4199c6.xml"}}, {"value": "0.02045", "module": "A1-A3"}, {"value": "2.791E-05", "module": "A4"}, {"value": "2.093E-05", "module": "A5"}, {"value": "1.411E-05", "module": "C1"}, {"value": "1.395E-05", "module": "C2"}, {"value": "0.005693", "module": "C3"}, {"value": "0", "module": "C4"}, {"value": "-0.004138", "module": "D"}]}}, {"referenceToLCIAMethodDataSet": {"shortDescription": [{"value": "Abiotic depletion potential for non fossil resources (ADPE)", "lang": "en"}], "type": "LCIA method data set", "refObjectId": "b2ad6494-c78d-11e6-9d9d-cec0c932ce01", "uri": "../lciamethods/b2ad6494-c78d-11e6-9d9d-cec0c932ce01.xml"}, "other": {"anies": [{"name": "referenceToUnitGroupDataSet", "value": {"shortDescription": [{"value": "kg Sb-Äq.", "lang": "en"}], "type": "unit group data set", "refObjectId": "54ccd2d9-a32a-4fc2-923d-f2c8c93e89d4", "uri": "../unitgroups/54ccd2d9-a32a-4fc2-923d-f2c8c93e89d4.xml"}}, {"value": "6.49E-06", "module": "A1-A3"}, {"value": "2.046E-09", "module": "A4"}, {"value": "8.601E-10", "module": "A5"}, {"value": "5.888E-11", "module": "C1"}, {"value": "1.023E-09", "module": "C2"}, {"value": "1.582E-08", "module": "C3"}, {"value": "0", "module": "C4"}, {"value": "-5.188E-07", "module": "D"}]}}, {"referenceToLCIAMethodDataSet": {"shortDescription": [{"value": "Abiotic depletion potential for fossil resources (ADPF)", "lang": "en"}], "type": "LCIA method data set", "refObjectId": "b2ad6110-c78d-11e6-9d9d-cec0c932ce01", "uri": "../lciamethods/b2ad6110-c78d-11e6-9d9d-cec0c932ce01.xml"}, "other": {"anies": [{"name": "referenceToUnitGroupDataSet", "value": {"shortDescription": [{"value": "MJ", "lang": "en"}], "type": "unit group data set", "refObjectId": "93a60a57-a3c8-11da-a746-0800200c9a66", "uri": "../unitgroups/93a60a57-a3c8-11da-a746-0800200c9a66.xml"}}, {"value": "188", "module": "A1-A3"}, {"value": "0.392", "module": "A4"}, {"value": "0.0791", "module": "A5"}, {"value": "0.0303", "module": "C1"}, {"value": "0.196", "module": "C2"}, {"value": "2.09", "module": "C3"}, {"value": "0", "module": "C4"}, {"value": "-57.5", "module": "D"}]}}, {"referenceToLCIAMethodDataSet": {"shortDescription": [{"value": "Water use (WDP)", "lang": "en"}], "type": "LCIA method data set", "refObjectId": "b2ad66ce-c78d-11e6-9d9d-cec0c932ce01", "uri": "../lciamethods/b2ad66ce-c78d-11e6-9d9d-cec0c932ce01.xml"}, "other": {"anies": [{"name": "referenceToUnitGroupDataSet", "value": {"shortDescription": [{"value": "m^(3) world-Äq. deprived", "lang": "en"}], "type": "unit group data set", "refObjectId": "6ae2df01-888e-46c8-b17d-49fa3869b476", "uri": "../unitgroups/6ae2df01-888e-46c8-b17d-49fa3869b476.xml"}}, {"value": "1135", "module": "A1-A3"}, {"value": "0.0006342", "module": "A4"}, {"value": "0.02078", "module": "A5"}, {"value": "3.909E-06", "module": "C1"}, {"value": "0.0003171", "module": "C2"}, {"value": "0.7582", "module": "C3"}, {"value": "0", "module": "C4"}, {"value": "-3.09", "module": "D"}]}}, {"referenceToLCIAMethodDataSet": {"shortDescription": [{"value": "Incidence of disease due to PM emissions (PM)", "lang": "en"}], "type": "LCIA method data set", "refObjectId": "b5c602c6-def3-11e6-bf01-fe55135034f3", "uri": "../lciamethods/b5c602c6-def3-11e6-bf01-fe55135034f3.xml"}, "other": {"anies": [{"name": "referenceToUnitGroupDataSet", "value": {"shortDescription": [{"value": "Disease incidence", "lang": "en"}], "type": "unit group data set", "refObjectId": "3883559b-648f-4afc-8ba2-0bd24f3affa3", "uri": "../unitgroups/3883559b-648f-4afc-8ba2-0bd24f3affa3.xml"}}, {"module": "A1-A3"}, {"module": "A4"}, {"module": "A5"}, {"module": "C1"}, {"module": "C2"}, {"module": "C3"}, {"module": "C4"}, {"module": "D"}]}}, {"referenceToLCIAMethodDataSet": {"shortDescription": [{"value": "Human exposure efficiency relative to U235 (IR)", "lang": "en"}], "type": "LCIA method data set", "refObjectId": "b5c632be-def3-11e6-bf01-fe55135034f3", "uri": "../lciamethods/b5c632be-def3-11e6-bf01-fe55135034f3.xml"}, "other": {"anies": [{"name": "referenceToUnitGroupDataSet", "value": {"shortDescription": [{"value": "kBq U235-Äq.", "lang": "en"}], "type": "unit group data set", "refObjectId": "456b05bf-1415-44a9-9993-02452f554c09", "uri": "../unitgroups/456b05bf-1415-44a9-9993-02452f554c09.xml"}}, {"module": "A1-A3"}, {"module": "A4"}, {"module": "A5"}, {"module": "C1"}, {"module": "C2"}, {"module": "C3"}, {"module": "C4"}, {"module": "D"}]}}, {"referenceToLCIAMethodDataSet": {"shortDescription": [{"value": "Comparative toxic unit for ecosystems (ETP-fw)", "lang": "en"}], "type": "LCIA method data set", "refObjectId": "ee1082d1-b0f7-43ca-a1f0-21e2a4a74511", "uri": "../lciamethods/ee1082d1-b0f7-43ca-a1f0-21e2a4a74511.xml"}, "other": {"anies": [{"name": "referenceToUnitGroupDataSet", "value": {"shortDescription": [{"value": "CTUe", "lang": "en"}], "type": "unit group data set", "refObjectId": "aa959ded-f1eb-4efb-9c5c-2d60be36b3e6", "uri": "../unitgroups/aa959ded-f1eb-4efb-9c5c-2d60be36b3e6.xml"}}, {"module": "A1-A3"}, {"module": "A4"}, {"module": "A5"}, {"module": "C1"}, {"module": "C2"}, {"module": "C3"}, {"module": "C4"}, {"module": "D"}]}}, {"referenceToLCIAMethodDataSet": {"shortDescription": [{"value": "Comparative toxic unit for humans (carcinogenic) (HTP-c)", "lang": "en"}], "type": "LCIA method data set", "refObjectId": "2299222a-bbd8-474f-9d4f-4dd1f18aea7c", "uri": "../lciamethods/2299222a-bbd8-474f-9d4f-4dd1f18aea7c.xml"}, "other": {"anies": [{"name": "referenceToUnitGroupDataSet", "value": {"shortDescription": [{"value": "CTUh", "lang": "en"}], "type": "unit group data set", "refObjectId": "d4c9523e-2d7e-49fd-8469-998f547d3a70", "uri": "../unitgroups/d4c9523e-2d7e-49fd-8469-998f547d3a70.xml"}}, {"module": "A1-A3"}, {"module": "A4"}, {"module": "A5"}, {"module": "C1"}, {"module": "C2"}, {"module": "C3"}, {"module": "C4"}, {"module": "D"}]}}, {"referenceToLCIAMethodDataSet": {"shortDescription": [{"value": "Comparative toxic unit for humans (noncarcinogenic) (HTP-nc)", "lang": "en"}], "type": "LCIA method data set", "refObjectId": "3af763a5-b7a1-48c9-9cee-1f223481fcef", "uri": "../lciamethods/3af763a5-b7a1-48c9-9cee-1f223481fcef.xml"}, "other": {"anies": [{"name": "referenceToUnitGroupDataSet", "value": {"shortDescription": [{"value": "CTUh", "lang": "en"}], "type": "unit group data set", "refObjectId": "d4c9523e-2d7e-49fd-8469-998f547d3a70", "uri": "../unitgroups/d4c9523e-2d7e-49fd-8469-998f547d3a70.xml"}}, {"module": "A1-A3"}, {"module": "A4"}, {"module": "A5"}, {"module": "C1"}, {"module": "C2"}, {"module": "C3"}, {"module": "C4"}, {"module": "D"}]}}, {"referenceToLCIAMethodDataSet": {"shortDescription": [{"value": "Soil quality index (SQP)", "lang": "en"}], "type": "LCIA method data set", "refObjectId": "b2ad6890-c78d-11e6-9d9d-cec0c932ce01", "uri": "../lciamethods/b2ad6890-c78d-11e6-9d9d-cec0c932ce01.xml"}, "other": {"anies": [{"name": "referenceToUnitGroupDataSet", "value": {"shortDescription": [{"value": "SQP", "lang": "en"}], "type": "unit group data set", "refObjectId": "f130951c-e67f-4f7f-8dd4-665de3974e18", "uri": "../unitgroups/f130951c-e67f-4f7f-8dd4-665de3974e18.xml"}}, {"module": "A1-A3"}, {"module": "A4"}, {"module": "A5"}, {"module": "C1"}, {"module": "C2"}, {"module": "C3"}, {"module": "C4"}, {"module": "D"}]}}]}, "otherAttributes": {"{http://www.indata.network/EPD/2019}epd-version": "1.2"}, "version": "1.1", "locations": "../ILCDLocations.xml"}