{"processInformation": {"dataSetInformation": {"UUID": "2db7a912-0462-4334-88aa-ec32c5059ca0", "name": {"baseName": [{"value": "Concrete ECOPact C30/37Cl02D16S3, Mix code 1133290, RMX Chitila plant, Romania", "lang": "en"}]}, "classificationInformation": {"classification": [{"class": [{"value": "Mineralische Baustoffe", "level": 0, "classId": "1"}, {"value": "Mörtel und Beton", "level": 1, "classId": "1.4"}, {"value": "Beton", "level": 2, "classId": "1.4.01"}], "name": "OEKOBAU.DAT"}, {"class": [{"value": "Bauprodukte", "level": 0}, {"value": "Normal- Leicht- und Porenbeton", "level": 1}, {"value": "Betonbauteile aus Ort- oder Lieferbeton", "level": 2}], "name": "IBUCategories"}]}, "generalComment": [{"value": "Concrete is produced by mixing cement, aggregates and water with potentially additional cementitious materials, fibers and additives.\n\nThe fresh concrete is generally poured into formwork, compacted and hardened in the desired form by hydration of the cement to form a solid artificial rock.\n", "lang": "en"}], "other": {"anies": [{"componentsAndMaterialsAndSubstances": [{"component": {"name": [{"value": "Cement", "lang": "en"}], "weightPerc": {"lowerValue": 10.0, "upperValue": 17.0}, "mass": {}}}, {"component": {"name": [{"value": "Water", "lang": "en"}], "weightPerc": {"lowerValue": 7.0, "upperValue": 10.0}, "mass": {}}}, {"component": {"name": [{"value": "Aggregate", "lang": "en"}], "weightPerc": {"lowerValue": 70.0, "upperValue": 90.0}, "mass": {}}}, {"component": {"name": [{"value": "Cementitious", "lang": "en"}], "weightPerc": {"lowerValue": 0.0, "upperValue": 1.0}, "mass": {}}}, {"component": {"name": [{"value": "Fibers", "lang": "en"}], "weightPerc": {"lowerValue": 0.0, "upperValue": 1.0}, "mass": {}}}, {"component": {"name": [{"value": "Admixtures", "lang": "en"}], "weightPerc": {"lowerValue": 0.0, "upperValue": 1.0}, "mass": {}}}]}, {"scenario": [{"description": [{"value": "100% Recycled", "lang": "en"}], "name": "Recycled", "group": "EoL", "default": true}, {"description": [{"value": "100% Landfill", "lang": "en"}], "name": "Landfill", "group": "EoL"}]}]}}, "quantitativeReference": {"referenceToReferenceFlow": [0]}, "time": {"referenceYear": 2025, "dataSetValidUntil": 2030, "timeRepresentativenessDescription": [{"value": "Annual average", "lang": "en"}], "other": {"anies": [{"name": "publicationDateOfEPD", "value": 1743120000000}]}}, "geography": {"locationOfOperationSupplyOrProduction": {"descriptionOfRestrictions": [{"value": "The data set represents production in the RMX Chitila plant of Holcim (Romania) SA in Romania", "lang": "en"}], "location": "RO"}}, "technology": {"technologyDescriptionAndIncludedProcesses": [{"value": "The dosed aggregates are first premixed with cement as a binding agent and other additives. The mixture is then mixed with water to form a plastically deformable fresh concrete. This is transported to the customer where it is placed in the prepared formwork and compacted.\n\nTo ensure the quality of the concrete, quality assurance systems is installed in RMX Chitila plant, which is based on the requirements for in-house production control in BS 8500 standard.", "lang": "en"}], "technologicalApplicability": [{"value": "Concrete is a widely used building material in the construction industry. It is used for example for the construction of walls, stairs, floor, foundations, bored piles or even complete structures such as bridges.", "lang": "en"}], "referenceToTechnologyFlowDiagrammOrPicture": [{"shortDescription": [{"lang": "en"}], "type": "source data set", "refObjectId": "86c27348-099a-4a5b-8093-fca99dcf61c8"}]}}, "modellingAndValidation": {"LCIMethodAndAllocation": {"typeOfDataSet": "EPD", "referenceToLCAMethodDetails": [{"shortDescription": [{"value": "PCR - Betonbauteile aus Ort- oder Lieferbeton/ Concrete components made of in-situ or ready-mixed concrete.pdf", "lang": "en"}], "type": "source data set", "refObjectId": "7d342877-0da7-4818-9724-903ccdfd600f", "version": "00.01.000"}], "other": {"anies": [{"name": "subType", "value": "specific dataset"}]}}, "dataSourcesTreatmentAndRepresentativeness": {"referenceToDataSource": [{"shortDescription": [{"value": "GaBi Database (SP40)", "lang": "en"}], "type": "source data set", "refObjectId": "28d74cc0-db8b-4d7e-bc44-5f6d56ce0c4a"}], "useAdviceForDataSet": [{"value": "This document refers to the production of ECOPact C30/37Cl02D16S3 concrete, mix code 1133290  produced in the plant of RMX Chitila of Holcim (Romania) SA for use as ready-mix concrete of normal building construction and civil engineering.\n\nType of EPD: cradle to gate with options, modules C1–C4, and module D (A1–A3 + C + D and additional modules A4, A5 and B1)\n\nThe selected system boundaries include the production of the concrete including the extraction of raw materials through to the installation, use and end of life of the finished product.\n\nModule A1: Extraction and processing of the raw materials used in concrete production\nModule A2: Transport of the raw materials to the plant\nModule A3: Concrete production in the plant and waste treatment\nModule A4: Transport to the construction site\nModule A5: Includes all processes associated with placing the concrete (e.g. pumping or installationby crane) as well as the production, transport and treatment of unused concrete (e.g. return concrete)\nModule B1: Carbonation during the use phase\nModule B2-B7: For concrete components, maintenance, repair refurbishment or replacement measures are not usually required during the reference service life. Therefore, no environmental burden is considered in these modules\nModule C1: Dismantling / demolition of concrete buildings / components\nModule C2: Transport of demolished concrete for processing\nModule C3: Concrete waste processing\nModule D: Benefits and loads for the use of concrete demolition waste as replacement for primary materials", "lang": "en"}], "other": {"anies": [{"name": "referenceToOriginalEPD", "value": {"shortDescription": {"value": "Concrete ECOPact C30/37Cl02D16S3, Mix code 1133290, RMX Chitila plant, Romania", "defaultValue": "Concrete ECOPact C30/37Cl02D16S3, Mix code 1133290, RMX Chitila plant, Romania", "lstrings": [{"lang": "en", "value": "Concrete ECOPact C30/37Cl02D16S3, Mix code 1133290, RMX Chitila plant, Romania"}]}, "version": {"version": 1000, "majorVersion": 0, "minorVersion": 1, "subMinorVersion": 0, "zero": false, "versionString": "00.01.000"}, "type": "source data set", "uuid": {"uuid": "2db7a912-0462-4334-88aa-ec32c5059ca0"}, "refObjectId": "2db7a912-0462-4334-88aa-ec32c5059ca0", "versionAsString": "00.01.000", "resourceURLs": ["https://oekobaudat.de/OEKOBAU.DAT/resource/sources/2db7a912-0462-4334-88aa-ec32c5059ca0/OriginalEPD.pdf?version=00.01.000"]}}]}}, "validation": {"review": [{"referenceToNameOfReviewerAndInstitution": [{"shortDescription": [{"value": "Matthias Schulz", "lang": "en"}], "type": "contact data set", "refObjectId": "8184d8aa-0045-43e5-a2c9-658acc9720de"}]}]}, "complianceDeclarations": {"compliance": [{"referenceToComplianceSystem": {"shortDescription": [{"value": "ISO 14025", "lang": "en"}], "type": "source data set", "refObjectId": "4f2eb655-6e44-4874-a95a-e28f5442cd4d"}}, {"referenceToComplianceSystem": {"shortDescription": [{"value": "EN 15804+A2", "lang": "en"}], "type": "source data set", "refObjectId": "c0016b33-8cf7-415c-ac6e-deba0d21440d"}}]}}, "administrativeInformation": {"dataGenerator": {"referenceToPersonOrEntityGeneratingTheDataSet": [{"shortDescription": [{"value": "Climate Earth, Inc.", "lang": "en"}], "type": "contact data set", "refObjectId": "4a3c46d9-30d8-4105-a89e-0e104067f5db"}]}, "dataEntryBy": {"timeStamp": 1743162149645, "referenceToDataSetFormat": [{"shortDescription": [{"value": "ILCD Format 1.1", "lang": "en"}], "type": "source data set", "refObjectId": "a97a0155-0234-4b87-b4ce-a45da52f2a40"}, {"shortDescription": [{"value": "EPD-Datenformaterweiterungen v1.2", "lang": "en"}], "type": "source data set", "refObjectId": "a29449fd-aa2f-4de8-b5d7-4b06b43c6fde"}], "referenceToPersonOrEntityEnteringTheData": {"shortDescription": [{"value": "Climate Earth, Inc.", "lang": "en"}], "type": "contact data set", "refObjectId": "4a3c46d9-30d8-4105-a89e-0e104067f5db"}}, "publicationAndOwnership": {"dataSetVersion": "00.01.000", "referenceToRegistrationAuthority": {"shortDescription": [{"value": "Institut Bauen und Umwelt e.V.", "lang": "en"}], "type": "contact data set", "refObjectId": "d111dbec-b024-4be5-86c5-752d6eb2cf95"}, "registrationNumber": "IBU-CEI-HOL-2205120-RO2025000086-ISUE001-EN", "referenceToOwnershipOfDataSet": {"shortDescription": [{"value": "Holcim (Romania) SA", "lang": "en"}], "type": "contact data set", "refObjectId": "0032ba6d-4d79-471c-aa3f-f487450c2ae8"}, "copyright": true, "licenseType": "Free of charge for all users and uses", "accessRestrictions": [{"value": "None", "lang": "en"}], "other": {"anies": [{"name": "referenceToPublisher", "value": {"shortDescription": [{"value": "Institut Bauen und Umwelt e. V.", "lang": "en"}], "type": "contact data set", "refObjectId": "d111dbec-b024-4be5-86c5-752d6eb2cf95"}}]}}}, "exchanges": {"exchange": [{"dataSetInternalID": 0, "referenceToFlowDataSet": {"shortDescription": [{"value": "Concrete ECOPact C30/37Cl02D16S3, Mix code 1133290, RMX Chitila plant, Romania", "lang": "en"}], "type": "flow data set", "refObjectId": "08ab56b0-3b00-466e-4e14-08dd6c743eda", "version": "00.01.000"}, "meanAmount": 1.0, "referenceFlow": true, "resultingflowAmount": 1.0, "flowProperties": [{"name": [{"lang": "en", "value": "Volume"}, {"lang": "de", "value": "Volumen"}], "uuid": "93a60a56-a3c8-22da-a746-0800200c9a66", "referenceFlowProperty": true, "meanValue": 1.0, "referenceUnit": "m3", "unitGroupUUID": "cd950537-0a98-4044-9ba7-9f9a68d0a504"}, {"name": [{"lang": "en", "value": "Mass"}], "uuid": "93a60a56-a3c8-11da-a746-0800200b9a66", "meanValue": 2335.59}], "materialProperties": [{"name": "layer thickness", "value": "0.2", "unit": "m", "unitDescription": "meters"}, {"name": "conversion factor to 1 kg", "value": "4.281573392590309E-4", "unit": "-", "unitDescription": "Without unit"}, {"name": "grammage", "value": "467.11800000000005", "unit": "kg/m^2", "unitDescription": "kilograms per square meter"}, {"name": "gross density", "value": "2335.59", "unit": "kg/m^3", "unitDescription": "kilograms per cubic metre"}], "typeOfFlow": "Product flow"}, {"dataSetInternalID": 1, "referenceToFlowDataSet": {"shortDescription": [{"value": "Use of renewable primary energy as energy carrier (PERE)", "lang": "en"}], "type": "flow data set", "refObjectId": "20f32be5-0398-4288-9b6d-accddd195317"}, "exchange direction": "INPUT", "other": {"anies": [{"name": "referenceToUnitGroupDataSet", "value": {"shortDescription": [{"value": "MJ", "lang": "en"}], "type": "unit group data set", "refObjectId": "93a60a57-a3c8-11da-a746-0800200c9a66"}}, {"value": "192.3614692650717", "module": "A1-A3"}, {"value": "0.8854170868118267", "module": "A4"}, {"value": "1.2002435488779972", "module": "A5"}, {"value": "0", "module": "B1"}, {"value": "0.742547377445982", "module": "C1"}, {"value": "1.0799945618638633", "module": "C2", "scenario": "Recycled"}, {"value": "1.0799945618638633", "module": "C2", "scenario": "Landfill"}, {"value": "8.868384462523052", "module": "C3", "scenario": "Recycled"}, {"value": "0", "module": "C3", "scenario": "Landfill"}, {"value": "0", "module": "C4", "scenario": "Recycled"}, {"value": "2.931094006003938", "module": "C4", "scenario": "Landfill"}, {"value": "-24.596575509215302", "module": "D", "scenario": "Recycled"}, {"value": "0", "module": "D", "scenario": "Landfill"}]}, "resolvedFlowVersion": "38.00.000", "flowProperties": [], "typeOfFlow": "Other flow", "classification": {"classHierarchy": "Quantities", "name": "GaBiCategories"}}, {"dataSetInternalID": 2, "referenceToFlowDataSet": {"shortDescription": [{"value": "Use of renewable primary energy resources used as raw materials (PERM)", "lang": "en"}], "type": "flow data set", "refObjectId": "fb3ec0de-548d-4508-aea5-00b73bf6f702"}, "exchange direction": "INPUT", "other": {"anies": [{"name": "referenceToUnitGroupDataSet", "value": {"shortDescription": [{"value": "MJ", "lang": "en"}], "type": "unit group data set", "refObjectId": "93a60a57-a3c8-11da-a746-0800200c9a66"}}, {"value": "23.3488580401", "module": "A1-A3"}, {"value": "0", "module": "A4"}, {"value": "0.08878677889319952", "module": "A5"}, {"value": "0", "module": "B1"}, {"value": "0", "module": "C1"}, {"value": "0", "module": "C2", "scenario": "Recycled"}, {"value": "0", "module": "C2", "scenario": "Landfill"}, {"value": "0", "module": "C3", "scenario": "Recycled"}, {"value": "0", "module": "C3", "scenario": "Landfill"}, {"value": "0", "module": "C4", "scenario": "Recycled"}, {"value": "0", "module": "C4", "scenario": "Landfill"}, {"value": "0", "module": "D", "scenario": "Recycled"}, {"value": "0", "module": "D", "scenario": "Landfill"}]}, "resolvedFlowVersion": "38.00.000", "flowProperties": [], "typeOfFlow": "Other flow", "classification": {"classHierarchy": "Quantities", "name": "GaBiCategories"}}, {"dataSetInternalID": 3, "referenceToFlowDataSet": {"shortDescription": [{"value": "Total use of renewable primary energy (PERT)", "lang": "en"}], "type": "flow data set", "refObjectId": "53f97275-fa8a-4cdd-9024-65936002acd0"}, "exchange direction": "INPUT", "other": {"anies": [{"name": "referenceToUnitGroupDataSet", "value": {"shortDescription": [{"value": "MJ", "lang": "en"}], "type": "unit group data set", "refObjectId": "93a60a57-a3c8-11da-a746-0800200c9a66"}}, {"value": "215.7284215150717", "module": "A1-A3"}, {"value": "0.8854170868118267", "module": "A4"}, {"value": "1.2890991331325072", "module": "A5"}, {"value": "0", "module": "B1"}, {"value": "0.742547377445982", "module": "C1"}, {"value": "1.0799945618638633", "module": "C2", "scenario": "Recycled"}, {"value": "1.0799945618638633", "module": "C2", "scenario": "Landfill"}, {"value": "8.868384462523052", "module": "C3", "scenario": "Recycled"}, {"value": "0", "module": "C3", "scenario": "Landfill"}, {"value": "0", "module": "C4", "scenario": "Recycled"}, {"value": "2.931094006003938", "module": "C4", "scenario": "Landfill"}, {"value": "-24.596575509215302", "module": "D", "scenario": "Recycled"}, {"value": "0", "module": "D", "scenario": "Landfill"}]}, "resolvedFlowVersion": "38.00.000", "flowProperties": [], "typeOfFlow": "Other flow", "classification": {"classHierarchy": "Quantities / Environmental quantities / EPD EN 15804 / LCI indicators", "name": "GaBiCategories"}}, {"dataSetInternalID": 4, "referenceToFlowDataSet": {"shortDescription": [{"value": "Use of non renewable primary energy as energy carrier (PENRE)", "lang": "en"}], "type": "flow data set", "refObjectId": "ac857178-2b45-46ec-892a-a9a4332f0372"}, "exchange direction": "INPUT", "other": {"anies": [{"name": "referenceToUnitGroupDataSet", "value": {"shortDescription": [{"value": "MJ", "lang": "en"}], "type": "unit group data set", "refObjectId": "93a60a57-a3c8-11da-a746-0800200c9a66"}}, {"value": "892.8760316286", "module": "A1-A3"}, {"value": "57.3247101934322", "module": "A4"}, {"value": "20.588436843032085", "module": "A5"}, {"value": "0", "module": "B1"}, {"value": "132.060926294238", "module": "C1"}, {"value": "97.12441658116387", "module": "C2", "scenario": "Recycled"}, {"value": "97.12441658116387", "module": "C2", "scenario": "Landfill"}, {"value": "64.36276296861061", "module": "C3", "scenario": "Recycled"}, {"value": "0", "module": "C3", "scenario": "Landfill"}, {"value": "0", "module": "C4", "scenario": "Recycled"}, {"value": "343.58485723560125", "module": "C4", "scenario": "Landfill"}, {"value": "-112.41707377541465", "module": "D", "scenario": "Recycled"}, {"value": "0", "module": "D", "scenario": "Landfill"}]}, "resolvedFlowVersion": "38.00.000", "flowProperties": [], "typeOfFlow": "Other flow", "classification": {"classHierarchy": "Quantities", "name": "GaBiCategories"}}, {"dataSetInternalID": 5, "referenceToFlowDataSet": {"shortDescription": [{"value": "Use of non renewable primary energy resources used as raw materials (PENRM)", "lang": "en"}], "type": "flow data set", "refObjectId": "1421caa0-679d-4bf4-b282-0eb850ccae27"}, "exchange direction": "INPUT", "other": {"anies": [{"name": "referenceToUnitGroupDataSet", "value": {"shortDescription": [{"value": "MJ", "lang": "en"}], "type": "unit group data set", "refObjectId": "93a60a57-a3c8-11da-a746-0800200c9a66"}}, {"value": "24.4854306409", "module": "A1-A3"}, {"value": "0", "module": "A4"}, {"value": "0.09310872988669085", "module": "A5"}, {"value": "0", "module": "B1"}, {"value": "0", "module": "C1"}, {"value": "0", "module": "C2", "scenario": "Recycled"}, {"value": "0", "module": "C2", "scenario": "Landfill"}, {"value": "0", "module": "C3", "scenario": "Recycled"}, {"value": "0", "module": "C3", "scenario": "Landfill"}, {"value": "0", "module": "C4", "scenario": "Recycled"}, {"value": "0", "module": "C4", "scenario": "Landfill"}, {"value": "0", "module": "D", "scenario": "Recycled"}, {"value": "0", "module": "D", "scenario": "Landfill"}]}, "resolvedFlowVersion": "38.00.000", "flowProperties": [], "typeOfFlow": "Other flow", "classification": {"classHierarchy": "Quantities", "name": "GaBiCategories"}}, {"dataSetInternalID": 6, "referenceToFlowDataSet": {"shortDescription": [{"value": "Total use of non renewable primary energy resource (PENRT)", "lang": "en"}], "type": "flow data set", "refObjectId": "06159210-646b-4c8d-8583-da9b3b95a6c1"}, "exchange direction": "INPUT", "other": {"anies": [{"name": "referenceToUnitGroupDataSet", "value": {"shortDescription": [{"value": "MJ", "lang": "en"}], "type": "unit group data set", "refObjectId": "93a60a57-a3c8-11da-a746-0800200c9a66"}}, {"value": "917.3607179886001", "module": "A1-A3"}, {"value": "57.3247101934322", "module": "A4"}, {"value": "20.68154274270311", "module": "A5"}, {"value": "0", "module": "B1"}, {"value": "132.060926294238", "module": "C1"}, {"value": "97.12441658116387", "module": "C2", "scenario": "Recycled"}, {"value": "97.12441658116387", "module": "C2", "scenario": "Landfill"}, {"value": "64.36276296861061", "module": "C3", "scenario": "Recycled"}, {"value": "0", "module": "C3", "scenario": "Landfill"}, {"value": "0", "module": "C4", "scenario": "Recycled"}, {"value": "343.58485723560125", "module": "C4", "scenario": "Landfill"}, {"value": "-112.41707377541465", "module": "D", "scenario": "Recycled"}, {"value": "0", "module": "D", "scenario": "Landfill"}]}, "resolvedFlowVersion": "38.00.000", "flowProperties": [], "typeOfFlow": "Other flow", "classification": {"classHierarchy": "Quantities / Environmental quantities / EPD EN 15804 / LCI indicators", "name": "GaBiCategories"}}, {"dataSetInternalID": 7, "referenceToFlowDataSet": {"shortDescription": [{"value": "Use of secondary material (SM)", "lang": "en"}], "type": "flow data set", "refObjectId": "c6a1f35f-2d09-4f54-8dfb-97e502e1ce92"}, "exchange direction": "INPUT", "other": {"anies": [{"name": "referenceToUnitGroupDataSet", "value": {"shortDescription": [{"value": "kg", "lang": "en"}], "type": "unit group data set", "refObjectId": "ad38d542-3fe9-439d-9b95-2f5f7752acaf"}}, {"value": "2.40149938079", "module": "A1-A3"}, {"value": "0", "module": "A4"}, {"value": "0.009131983849838168", "module": "A5"}, {"value": "0", "module": "B1"}, {"value": "0", "module": "C1"}, {"value": "0", "module": "C2", "scenario": "Recycled"}, {"value": "0", "module": "C2", "scenario": "Landfill"}, {"value": "0", "module": "C3", "scenario": "Recycled"}, {"value": "0", "module": "C3", "scenario": "Landfill"}, {"value": "0", "module": "C4", "scenario": "Recycled"}, {"value": "0", "module": "C4", "scenario": "Landfill"}, {"value": "2333.19763260306", "module": "D", "scenario": "Recycled"}, {"value": "0", "module": "D", "scenario": "Landfill"}]}, "resolvedFlowVersion": "38.00.000", "flowProperties": [], "typeOfFlow": "Other flow", "classification": {"classHierarchy": "Quantities / Environmental quantities / EPD EN 15804 / LCI indicators", "name": "GaBiCategories"}}, {"dataSetInternalID": 8, "referenceToFlowDataSet": {"shortDescription": [{"value": "Use of renewable secondary fuels (RSF)", "lang": "en"}], "type": "flow data set", "refObjectId": "64333088-a55f-4aa2-9a31-c10b07816787"}, "exchange direction": "INPUT", "other": {"anies": [{"name": "referenceToUnitGroupDataSet", "value": {"shortDescription": [{"value": "MJ", "lang": "en"}], "type": "unit group data set", "refObjectId": "93a60a57-a3c8-11da-a746-0800200c9a66"}}, {"value": "305.99", "module": "A1-A3"}, {"value": "0", "module": "A4"}, {"value": "1.1635629642730811", "module": "A5"}, {"value": "0", "module": "B1"}, {"value": "0", "module": "C1"}, {"value": "0", "module": "C2", "scenario": "Recycled"}, {"value": "0", "module": "C2", "scenario": "Landfill"}, {"value": "0", "module": "C3", "scenario": "Recycled"}, {"value": "0", "module": "C3", "scenario": "Landfill"}, {"value": "0", "module": "C4", "scenario": "Recycled"}, {"value": "0", "module": "C4", "scenario": "Landfill"}, {"value": "0", "module": "D", "scenario": "Recycled"}, {"value": "0", "module": "D", "scenario": "Landfill"}]}, "resolvedFlowVersion": "38.00.000", "flowProperties": [], "typeOfFlow": "Other flow", "classification": {"classHierarchy": "Quantities / Environmental quantities / EPD EN 15804 / LCI indicators", "name": "GaBiCategories"}}, {"dataSetInternalID": 9, "referenceToFlowDataSet": {"shortDescription": [{"value": "Use of non renewable secondary fuels (NRSF)", "lang": "en"}], "type": "flow data set", "refObjectId": "89def144-d39a-4287-b86f-efde453ddcb2"}, "exchange direction": "INPUT", "other": {"anies": [{"name": "referenceToUnitGroupDataSet", "value": {"shortDescription": [{"value": "MJ", "lang": "en"}], "type": "unit group data set", "refObjectId": "93a60a57-a3c8-11da-a746-0800200c9a66"}}, {"value": "321.15999999999997", "module": "A1-A3"}, {"value": "0", "module": "A4"}, {"value": "1.2212486735054828", "module": "A5"}, {"value": "0", "module": "B1"}, {"value": "0", "module": "C1"}, {"value": "0", "module": "C2", "scenario": "Recycled"}, {"value": "0", "module": "C2", "scenario": "Landfill"}, {"value": "0", "module": "C3", "scenario": "Recycled"}, {"value": "0", "module": "C3", "scenario": "Landfill"}, {"value": "0", "module": "C4", "scenario": "Recycled"}, {"value": "0", "module": "C4", "scenario": "Landfill"}, {"value": "0", "module": "D", "scenario": "Recycled"}, {"value": "0", "module": "D", "scenario": "Landfill"}]}, "resolvedFlowVersion": "38.00.000", "flowProperties": [], "typeOfFlow": "Other flow", "classification": {"classHierarchy": "Quantities / Environmental quantities / EPD EN 15804 / LCI indicators", "name": "GaBiCategories"}}, {"dataSetInternalID": 10, "referenceToFlowDataSet": {"shortDescription": [{"value": "Net use of fresh water (FW)", "lang": "en"}], "type": "flow data set", "refObjectId": "3cf952c8-f3a4-461d-8c96-96456ca62246"}, "exchange direction": "INPUT", "other": {"anies": [{"name": "referenceToUnitGroupDataSet", "value": {"shortDescription": [{"value": "m^3", "lang": "en"}], "type": "unit group data set", "refObjectId": "cd950537-0a98-4044-9ba7-9f9a68d0a504"}}, {"value": "3.239573129556819", "module": "A1-A3"}, {"value": "0.00887663303602482", "module": "A4"}, {"value": "0.015010540567729557", "module": "A5"}, {"value": "0", "module": "B1"}, {"value": "0.00646624552453558", "module": "C1"}, {"value": "0.011029666037709877", "module": "C2", "scenario": "Recycled"}, {"value": "0.011029666037709877", "module": "C2", "scenario": "Landfill"}, {"value": "0.04848288490377", "module": "C3", "scenario": "Recycled"}, {"value": "0", "module": "C3", "scenario": "Landfill"}, {"value": "0", "module": "C4", "scenario": "Recycled"}, {"value": "0.36474097793910254", "module": "C4", "scenario": "Landfill"}, {"value": "-1.830996816690184", "module": "D", "scenario": "Recycled"}, {"value": "0", "module": "D", "scenario": "Landfill"}]}, "resolvedFlowVersion": "38.00.000", "flowProperties": [], "typeOfFlow": "Other flow", "classification": {"classHierarchy": "Quantities / Environmental quantities / EPD EN 15804 / LCI indicators", "name": "GaBiCategories"}}, {"dataSetInternalID": 11, "referenceToFlowDataSet": {"shortDescription": [{"value": "Hazardous waste disposed (HWD)", "lang": "en"}], "type": "flow data set", "refObjectId": "430f9e0f-59b2-46a0-8e0d-55e0e84948fc"}, "exchange direction": "OUTPUT", "other": {"anies": [{"name": "referenceToUnitGroupDataSet", "value": {"shortDescription": [{"value": "kg", "lang": "en"}], "type": "unit group data set", "refObjectId": "ad38d542-3fe9-439d-9b95-2f5f7752acaf"}}, {"value": "0.82574049696863", "module": "A1-A3"}, {"value": "0.04521661761258961", "module": "A4"}, {"value": "0.014638099498170593", "module": "A5"}, {"value": "0", "module": "B1"}, {"value": "0.104665507713135", "module": "C1"}, {"value": "0.08679567878281809", "module": "C2", "scenario": "Recycled"}, {"value": "0.08679567878281809", "module": "C2", "scenario": "Landfill"}, {"value": "0.14463132900435002", "module": "C3", "scenario": "Recycled"}, {"value": "0", "module": "C3", "scenario": "Landfill"}, {"value": "0", "module": "C4", "scenario": "Recycled"}, {"value": "0.23248006946772617", "module": "C4", "scenario": "Landfill"}, {"value": "-0.7610310737947621", "module": "D", "scenario": "Recycled"}, {"value": "0", "module": "D", "scenario": "Landfill"}]}, "resolvedFlowVersion": "38.00.000", "flowProperties": [], "typeOfFlow": "Other flow", "classification": {"classHierarchy": "Quantities / Environmental quantities / EPD EN 15804 / LCI indicators", "name": "GaBiCategories"}}, {"dataSetInternalID": 12, "referenceToFlowDataSet": {"shortDescription": [{"value": "Non harzardous waste disposed (NHWD)", "lang": "en"}], "type": "flow data set", "refObjectId": "b29ef66b-e286-4afa-949f-62f1a7b4d7fa"}, "exchange direction": "OUTPUT", "other": {"anies": [{"name": "referenceToUnitGroupDataSet", "value": {"shortDescription": [{"value": "kg", "lang": "en"}], "type": "unit group data set", "refObjectId": "ad38d542-3fe9-439d-9b95-2f5f7752acaf"}}, {"value": "35.52491341422392", "module": "A1-A3"}, {"value": "3.6571419929489943", "module": "A4"}, {"value": "0.2619011174252911", "module": "A5"}, {"value": "0", "module": "B1"}, {"value": "0.550137505086221", "module": "C1"}, {"value": "9.586391361856926", "module": "C2", "scenario": "Recycled"}, {"value": "9.586391361856926", "module": "C2", "scenario": "Landfill"}, {"value": "1.2086735121616503", "module": "C3", "scenario": "Recycled"}, {"value": "0", "module": "C3", "scenario": "Landfill"}, {"value": "0", "module": "C4", "scenario": "Recycled"}, {"value": "2336.6051482905614", "module": "C4", "scenario": "Landfill"}, {"value": "-7.681217096974338", "module": "D", "scenario": "Recycled"}, {"value": "0", "module": "D", "scenario": "Landfill"}]}, "resolvedFlowVersion": "38.00.000", "flowProperties": [], "typeOfFlow": "Other flow", "classification": {"classHierarchy": "Quantities / Environmental quantities / EPD EN 15804 / LCI indicators", "name": "GaBiCategories"}}, {"dataSetInternalID": 13, "referenceToFlowDataSet": {"shortDescription": [{"value": "Radioactive waste disposed (RWD)", "lang": "en"}], "type": "flow data set", "refObjectId": "3449546e-52ad-4b39-b809-9fb77cea8ff6"}, "exchange direction": "OUTPUT", "other": {"anies": [{"name": "referenceToUnitGroupDataSet", "value": {"shortDescription": [{"value": "kg", "lang": "en"}], "type": "unit group data set", "refObjectId": "ad38d542-3fe9-439d-9b95-2f5f7752acaf"}}, {"value": "0.008047637499033637", "module": "A1-A3"}, {"value": "0.0003854305262784894", "module": "A4"}, {"value": "0.0001639703645510502", "module": "A5"}, {"value": "0", "module": "B1"}, {"value": "0.000911792349721218", "module": "C1"}, {"value": "0.0006427363192019532", "module": "C2", "scenario": "Recycled"}, {"value": "0.0006427363192019532", "module": "C2", "scenario": "Landfill"}, {"value": "0.00070769778354", "module": "C3", "scenario": "Recycled"}, {"value": "0", "module": "C3", "scenario": "Landfill"}, {"value": "0", "module": "C4", "scenario": "Recycled"}, {"value": "0.0022515305579293298", "module": "C4", "scenario": "Landfill"}, {"value": "-0.0013589032983783067", "module": "D", "scenario": "Recycled"}, {"value": "0", "module": "D", "scenario": "Landfill"}]}, "resolvedFlowVersion": "38.00.000", "flowProperties": [], "typeOfFlow": "Other flow", "classification": {"classHierarchy": "Quantities / Environmental quantities / EPD EN 15804 / LCI indicators", "name": "GaBiCategories"}}, {"dataSetInternalID": 14, "referenceToFlowDataSet": {"shortDescription": [{"value": "Components for re-use (CRU)", "lang": "en"}], "type": "flow data set", "refObjectId": "a2b32f97-3fc7-4af2-b209-525bc6426f33"}, "exchange direction": "OUTPUT", "other": {"anies": [{"name": "referenceToUnitGroupDataSet", "value": {"shortDescription": [{"value": "kg", "lang": "en"}], "type": "unit group data set", "refObjectId": "ad38d542-3fe9-439d-9b95-2f5f7752acaf"}}, {"value": "0", "module": "A1-A3"}, {"value": "0", "module": "A4"}, {"value": "0", "module": "A5"}, {"value": "0", "module": "B1"}, {"value": "0", "module": "C1"}, {"value": "0", "module": "C2", "scenario": "Recycled"}, {"value": "0", "module": "C2", "scenario": "Landfill"}, {"value": "0", "module": "C3", "scenario": "Recycled"}, {"value": "0", "module": "C3", "scenario": "Landfill"}, {"value": "0", "module": "C4", "scenario": "Recycled"}, {"value": "0", "module": "C4", "scenario": "Landfill"}, {"value": "0", "module": "D", "scenario": "Recycled"}, {"value": "0", "module": "D", "scenario": "Landfill"}]}, "resolvedFlowVersion": "38.00.000", "flowProperties": [], "typeOfFlow": "Other flow", "classification": {"classHierarchy": "Quantities / Environmental quantities / EPD EN 15804 / LCI indicators", "name": "GaBiCategories"}}, {"dataSetInternalID": 15, "referenceToFlowDataSet": {"shortDescription": [{"value": "Materials for recycling (MFR)", "lang": "en"}], "type": "flow data set", "refObjectId": "d7fe48a5-4103-49c8-9aae-b0b5dfdbd6ae"}, "exchange direction": "OUTPUT", "other": {"anies": [{"name": "referenceToUnitGroupDataSet", "value": {"shortDescription": [{"value": "kg", "lang": "en"}], "type": "unit group data set", "refObjectId": "ad38d542-3fe9-439d-9b95-2f5f7752acaf"}}, {"value": "0.125595649", "module": "A1-A3"}, {"value": "0", "module": "A4"}, {"value": "0.0004775922273611603", "module": "A5"}, {"value": "0", "module": "B1"}, {"value": "0", "module": "C1"}, {"value": "0", "module": "C2", "scenario": "Recycled"}, {"value": "0", "module": "C2", "scenario": "Landfill"}, {"value": "2335.59", "module": "C3", "scenario": "Recycled"}, {"value": "0", "module": "C3", "scenario": "Landfill"}, {"value": "0", "module": "C4", "scenario": "Recycled"}, {"value": "0", "module": "C4", "scenario": "Landfill"}, {"value": "0", "module": "D", "scenario": "Recycled"}, {"value": "0", "module": "D", "scenario": "Landfill"}]}, "resolvedFlowVersion": "38.00.000", "flowProperties": [], "typeOfFlow": "Other flow", "classification": {"classHierarchy": "Quantities / Environmental quantities / EPD EN 15804 / LCI indicators", "name": "GaBiCategories"}}, {"dataSetInternalID": 16, "referenceToFlowDataSet": {"shortDescription": [{"value": "Materials for energy recovery (MER)", "lang": "en"}], "type": "flow data set", "refObjectId": "59a9181c-3aaf-46ee-8b13-2b3723b6e447"}, "exchange direction": "OUTPUT", "other": {"anies": [{"name": "referenceToUnitGroupDataSet", "value": {"shortDescription": [{"value": "kg", "lang": "en"}], "type": "unit group data set", "refObjectId": "ad38d542-3fe9-439d-9b95-2f5f7752acaf"}}, {"value": "0", "module": "A1-A3"}, {"value": "0", "module": "A4"}, {"value": "0", "module": "A5"}, {"value": "0", "module": "B1"}, {"value": "0", "module": "C1"}, {"value": "0", "module": "C2", "scenario": "Recycled"}, {"value": "0", "module": "C2", "scenario": "Landfill"}, {"value": "0", "module": "C3", "scenario": "Recycled"}, {"value": "0", "module": "C3", "scenario": "Landfill"}, {"value": "0", "module": "C4", "scenario": "Recycled"}, {"value": "0", "module": "C4", "scenario": "Landfill"}, {"value": "0", "module": "D", "scenario": "Recycled"}, {"value": "0", "module": "D", "scenario": "Landfill"}]}, "resolvedFlowVersion": "38.00.000", "flowProperties": [], "typeOfFlow": "Other flow", "classification": {"classHierarchy": "Quantities / Environmental quantities / EPD EN 15804 / LCI indicators", "name": "GaBiCategories"}}, {"dataSetInternalID": 17, "referenceToFlowDataSet": {"shortDescription": [{"value": "Exported electrical energy (EEE)", "lang": "en"}], "type": "flow data set", "refObjectId": "4da0c987-2b76-40d6-9e9e-82a017aaaf29"}, "exchange direction": "OUTPUT", "other": {"anies": [{"name": "referenceToUnitGroupDataSet", "value": {"shortDescription": [{"value": "MJ", "lang": "en"}], "type": "unit group data set", "refObjectId": "93a60a57-a3c8-11da-a746-0800200c9a66"}}, {"value": "0", "module": "A1-A3"}, {"value": "0", "module": "A4"}, {"value": "0", "module": "A5"}, {"value": "0", "module": "B1"}, {"value": "0", "module": "C1"}, {"value": "0", "module": "C2", "scenario": "Recycled"}, {"value": "0", "module": "C2", "scenario": "Landfill"}, {"value": "0", "module": "C3", "scenario": "Recycled"}, {"value": "0", "module": "C3", "scenario": "Landfill"}, {"value": "0", "module": "C4", "scenario": "Recycled"}, {"value": "0", "module": "C4", "scenario": "Landfill"}, {"value": "0", "module": "D", "scenario": "Recycled"}, {"value": "0", "module": "D", "scenario": "Landfill"}]}, "resolvedFlowVersion": "38.00.000", "flowProperties": [], "typeOfFlow": "Other flow", "classification": {"classHierarchy": "Quantities / Environmental quantities / EPD EN 15804 / LCI indicators", "name": "GaBiCategories"}}, {"dataSetInternalID": 18, "referenceToFlowDataSet": {"shortDescription": [{"value": "Exported thermal energy (EET)", "lang": "en"}], "type": "flow data set", "refObjectId": "98daf38a-7a79-46d3-9a37-2b7bd0955810"}, "exchange direction": "OUTPUT", "other": {"anies": [{"name": "referenceToUnitGroupDataSet", "value": {"shortDescription": [{"value": "MJ", "lang": "en"}], "type": "unit group data set", "refObjectId": "93a60a57-a3c8-11da-a746-0800200c9a66"}}, {"value": "0", "module": "A1-A3"}, {"value": "0", "module": "A4"}, {"value": "0", "module": "A5"}, {"value": "0", "module": "B1"}, {"value": "0", "module": "C1"}, {"value": "0", "module": "C2", "scenario": "Recycled"}, {"value": "0", "module": "C2", "scenario": "Landfill"}, {"value": "0", "module": "C3", "scenario": "Recycled"}, {"value": "0", "module": "C3", "scenario": "Landfill"}, {"value": "0", "module": "C4", "scenario": "Recycled"}, {"value": "0", "module": "C4", "scenario": "Landfill"}, {"value": "0", "module": "D", "scenario": "Recycled"}, {"value": "0", "module": "D", "scenario": "Landfill"}]}, "resolvedFlowVersion": "38.00.000", "flowProperties": [], "typeOfFlow": "Other flow", "classification": {"classHierarchy": "Quantities / Environmental quantities / EPD EN 15804 / LCI indicators", "name": "GaBiCategories"}}]}, "LCIAResults": {"LCIAResult": [{"referenceToLCIAMethodDataSet": {"shortDescription": [{"value": "Global Warming Potential - total (GWP-total)", "lang": "en"}], "type": "LCIA method data set", "refObjectId": "6a37f984-a4b3-458a-a20a-64418c145fa2"}, "other": {"anies": [{"name": "referenceToUnitGroupDataSet", "value": {"shortDescription": [{"value": "kg CO_(2) eqv.", "lang": "en"}], "type": "unit group data set", "refObjectId": "1ebf3012-d0db-4de2-aefd-ef30cedb0be1"}}, {"value": "186.40817048042376", "module": "A1-A3"}, {"value": "3.7578073907869465", "module": "A4"}, {"value": "1.8951266307291599", "module": "A5"}, {"value": "-6.423417546132803", "module": "B1"}, {"value": "9.53185574930846", "module": "C1"}, {"value": "6.2909133336175875", "module": "C2", "scenario": "Recycled"}, {"value": "6.2909133336175875", "module": "C2", "scenario": "Landfill"}, {"value": "-0.1132735790572097", "module": "C3", "scenario": "Recycled"}, {"value": "0", "module": "C3", "scenario": "Landfill"}, {"value": "0", "module": "C4", "scenario": "Recycled"}, {"value": "8.397788350307085", "module": "C4", "scenario": "Landfill"}, {"value": "-8.304093890271204", "module": "D", "scenario": "Recycled"}, {"value": "0", "module": "D", "scenario": "Landfill"}]}}, {"referenceToLCIAMethodDataSet": {"shortDescription": [{"value": "Global Warming Potential - fossil fuels (GWP-fossil)", "lang": "en"}], "type": "LCIA method data set", "refObjectId": "5f635281-343e-44fb-83df-1971b155e6b6"}, "other": {"anies": [{"name": "referenceToUnitGroupDataSet", "value": {"shortDescription": [{"value": "kg CO_(2) eqv.", "lang": "en"}], "type": "unit group data set", "refObjectId": "1ebf3012-d0db-4de2-aefd-ef30cedb0be1"}}, {"value": "186.164797375326", "module": "A1-A3"}, {"value": "3.754648637742283", "module": "A4"}, {"value": "1.8939886891844768", "module": "A5"}, {"value": "-6.423417546132803", "module": "B1"}, {"value": "9.52959739731502", "module": "C1"}, {"value": "6.286755389943883", "module": "C2", "scenario": "Recycled"}, {"value": "6.286755389943883", "module": "C2", "scenario": "Landfill"}, {"value": "-0.11441805319105969", "module": "C3", "scenario": "Recycled"}, {"value": "0", "module": "C3", "scenario": "Landfill"}, {"value": "0", "module": "C4", "scenario": "Recycled"}, {"value": "8.380685646291262", "module": "C4", "scenario": "Landfill"}, {"value": "-8.273564598880386", "module": "D", "scenario": "Recycled"}, {"value": "0", "module": "D", "scenario": "Landfill"}]}}, {"referenceToLCIAMethodDataSet": {"shortDescription": [{"value": "Global Warming Potential - biogenic (GWP-biogenic)", "lang": "en"}], "type": "LCIA method data set", "refObjectId": "2356e1ab-0185-4db5-86e5-16de51c7485c"}, "other": {"anies": [{"name": "referenceToUnitGroupDataSet", "value": {"shortDescription": [{"value": "kg CO_(2) eqv.", "lang": "en"}], "type": "unit group data set", "refObjectId": "1ebf3012-d0db-4de2-aefd-ef30cedb0be1"}}, {"value": "0.21943503677489704", "module": "A1-A3"}, {"value": "0.00164111884964256", "module": "A4"}, {"value": "0.000982036114973572", "module": "A5"}, {"value": "0", "module": "B1"}, {"value": "0.00124916493553934", "module": "C1"}, {"value": "0.0017195217212859807", "module": "C2", "scenario": "Recycled"}, {"value": "0.0017195217212859807", "module": "C2", "scenario": "Landfill"}, {"value": "0.0009343224168300001", "module": "C3", "scenario": "Recycled"}, {"value": "0", "module": "C3", "scenario": "Landfill"}, {"value": "0", "module": "C4", "scenario": "Recycled"}, {"value": "0.005497514775952408", "module": "C4", "scenario": "Landfill"}, {"value": "-0.026155686763331066", "module": "D", "scenario": "Recycled"}, {"value": "0", "module": "D", "scenario": "Landfill"}]}}, {"referenceToLCIAMethodDataSet": {"shortDescription": [{"value": "Global Warming Potential - land use and land use change (GWP-luluc)", "lang": "en"}], "type": "LCIA method data set", "refObjectId": "4331bbdb-978a-490d-8707-eeb047f01a55"}, "other": {"anies": [{"name": "referenceToUnitGroupDataSet", "value": {"shortDescription": [{"value": "kg CO_(2) eqv.", "lang": "en"}], "type": "unit group data set", "refObjectId": "1ebf3012-d0db-4de2-aefd-ef30cedb0be1"}}, {"value": "0.018440651577292945", "module": "A1-A3"}, {"value": "0.0016444798569910746", "module": "A4"}, {"value": "0.00015226856710070299", "module": "A5"}, {"value": "0", "module": "B1"}, {"value": "0.00100918705786836", "module": "C1"}, {"value": "0.0024384219524222896", "module": "C2", "scenario": "Recycled"}, {"value": "0.0024384219524222896", "module": "C2", "scenario": "Landfill"}, {"value": "0.00034313086926000006", "module": "C3", "scenario": "Recycled"}, {"value": "0", "module": "C3", "scenario": "Landfill"}, {"value": "0", "module": "C4", "scenario": "Recycled"}, {"value": "0.011605189239902945", "module": "C4", "scenario": "Landfill"}, {"value": "-0.004885902498481415", "module": "D", "scenario": "Recycled"}, {"value": "0", "module": "D", "scenario": "Landfill"}]}}, {"referenceToLCIAMethodDataSet": {"shortDescription": [{"value": "Depletion potential of the stratospheric ozone layer (ODP)", "lang": "en"}], "type": "LCIA method data set", "refObjectId": "b5c629d6-def3-11e6-bf01-fe55135034f3"}, "other": {"anies": [{"name": "referenceToUnitGroupDataSet", "value": {"shortDescription": [{"value": "kg CFC11 eqv.", "lang": "en"}], "type": "unit group data set", "refObjectId": "d9e957c9-7309-4474-bf3a-7777df6c4e5b"}}, {"value": "9.515726135432085E-06", "module": "A1-A3"}, {"value": "8.688512246162308E-07", "module": "A4"}, {"value": "2.856764762374013E-07", "module": "A5"}, {"value": "0", "module": "B1"}, {"value": "2.05778013828882E-06", "module": "C1"}, {"value": "1.4319235189864452E-06", "module": "C2", "scenario": "Recycled"}, {"value": "1.4319235189864452E-06", "module": "C2", "scenario": "Landfill"}, {"value": "5.086821596400001E-07", "module": "C3", "scenario": "Recycled"}, {"value": "0", "module": "C3", "scenario": "Landfill"}, {"value": "0", "module": "C4", "scenario": "Recycled"}, {"value": "4.975928630212458E-06", "module": "C4", "scenario": "Landfill"}, {"value": "-8.580637609589991E-07", "module": "D", "scenario": "Recycled"}, {"value": "0", "module": "D", "scenario": "Landfill"}]}}, {"referenceToLCIAMethodDataSet": {"shortDescription": [{"value": "Acidification potential, Accumulated Exceedance (AP)", "lang": "en"}], "type": "LCIA method data set", "refObjectId": "b5c611c6-def3-11e6-bf01-fe55135034f3"}, "other": {"anies": [{"name": "referenceToUnitGroupDataSet", "value": {"shortDescription": [{"value": "mol H^(+) eqv.", "lang": "en"}], "type": "unit group data set", "refObjectId": "42e089ac-92bf-4bf2-8ca1-5fc40d18f2ed"}}, {"value": "0.5551770978687499", "module": "A1-A3"}, {"value": "0.010977318627191942", "module": "A4"}, {"value": "0.014229363180983893", "module": "A5"}, {"value": "0", "module": "B1"}, {"value": "0.100035429998281", "module": "C1"}, {"value": "0.026713446133922254", "module": "C2", "scenario": "Recycled"}, {"value": "0.026713446133922254", "module": "C2", "scenario": "Landfill"}, {"value": "0.0313463037285", "module": "C3", "scenario": "Recycled"}, {"value": "0", "module": "C3", "scenario": "Landfill"}, {"value": "0", "module": "C4", "scenario": "Recycled"}, {"value": "0.11566288822628086", "module": "C4", "scenario": "Landfill"}, {"value": "-0.07652015619023443", "module": "D", "scenario": "Recycled"}, {"value": "0", "module": "D", "scenario": "Landfill"}]}}, {"referenceToLCIAMethodDataSet": {"shortDescription": [{"value": "Eutrophication potential - freshwater (EP-freshwater)", "lang": "en"}], "type": "LCIA method data set", "refObjectId": "b53ec18f-7377-4ad3-86eb-cc3f4f276b2b"}, "other": {"anies": [{"name": "referenceToUnitGroupDataSet", "value": {"shortDescription": [{"value": "kg P eqv.", "lang": "en"}], "type": "unit group data set", "refObjectId": "0429039d-a61d-4590-ba67-aa4a20a810a1"}}, {"value": "0.00885942776178654", "module": "A1-A3"}, {"value": "0.0002681499850081301", "module": "A4"}, {"value": "7.825956374780263E-05", "module": "A5"}, {"value": "0", "module": "B1"}, {"value": "0.000298246684413964", "module": "C1"}, {"value": "0.0004596638768710633", "module": "C2", "scenario": "Recycled"}, {"value": "0.0004596638768710633", "module": "C2", "scenario": "Landfill"}, {"value": "0.0005838554593800001", "module": "C3", "scenario": "Recycled"}, {"value": "0", "module": "C3", "scenario": "Landfill"}, {"value": "0", "module": "C4", "scenario": "Recycled"}, {"value": "0.001126061560201184", "module": "C4", "scenario": "Landfill"}, {"value": "-0.002072110484317145", "module": "D", "scenario": "Recycled"}, {"value": "0", "module": "D", "scenario": "Landfill"}]}}, {"referenceToLCIAMethodDataSet": {"shortDescription": [{"value": "Eutrophication potential - marine (EP-marine)", "lang": "en"}], "type": "LCIA method data set", "refObjectId": "b5c619fa-def3-11e6-bf01-fe55135034f3"}, "other": {"anies": [{"name": "referenceToUnitGroupDataSet", "value": {"shortDescription": [{"value": "kg N eqv.", "lang": "en"}], "type": "unit group data set", "refObjectId": "d05bb823-ecdf-4686-8c40-bf1d9257859f"}}, {"value": "0.18636881275505687", "module": "A1-A3"}, {"value": "0.002253286336608466", "module": "A4"}, {"value": "0.0059395839598782784", "module": "A5"}, {"value": "0", "module": "B1"}, {"value": "0.0443147602935876", "module": "C1"}, {"value": "0.008053001624634076", "module": "C2", "scenario": "Recycled"}, {"value": "0.008053001624634076", "module": "C2", "scenario": "Landfill"}, {"value": "0.010598865379380002", "module": "C3", "scenario": "Recycled"}, {"value": "0", "module": "C3", "scenario": "Landfill"}, {"value": "0", "module": "C4", "scenario": "Recycled"}, {"value": "0.04020802131273868", "module": "C4", "scenario": "Landfill"}, {"value": "-0.01842260652576046", "module": "D", "scenario": "Recycled"}, {"value": "0", "module": "D", "scenario": "Landfill"}]}}, {"referenceToLCIAMethodDataSet": {"shortDescription": [{"value": "Eutrophication potential - terrestrial (EP-terrestrial)", "lang": "en"}], "type": "LCIA method data set", "refObjectId": "b5c614d2-def3-11e6-bf01-fe55135034f3"}, "other": {"anies": [{"name": "referenceToUnitGroupDataSet", "value": {"shortDescription": [{"value": "mol N eqv.", "lang": "en"}], "type": "unit group data set", "refObjectId": "71b4d617-0ec9-4d3f-b65e-e438940c2401"}}, {"value": "2.106571317489463", "module": "A1-A3"}, {"value": "0.024533501441063855", "module": "A4"}, {"value": "0.06528319066128727", "module": "A5"}, {"value": "0", "module": "B1"}, {"value": "0.485511948540883", "module": "C1"}, {"value": "0.08799904048467375", "module": "C2", "scenario": "Recycled"}, {"value": "0.08799904048467375", "module": "C2", "scenario": "Landfill"}, {"value": "0.11473789071330001", "module": "C3", "scenario": "Recycled"}, {"value": "0", "module": "C3", "scenario": "Landfill"}, {"value": "0", "module": "C4", "scenario": "Recycled"}, {"value": "0.4402533996579883", "module": "C4", "scenario": "Landfill"}, {"value": "-0.23112647115734672", "module": "D", "scenario": "Recycled"}, {"value": "0", "module": "D", "scenario": "Landfill"}]}}, {"referenceToLCIAMethodDataSet": {"shortDescription": [{"value": "Photochemical Ozone Creation Potential  (POCP)", "lang": "en"}], "type": "LCIA method data set", "refObjectId": "b5c610fe-def3-11e6-bf01-fe55135034f3"}, "other": {"anies": [{"name": "referenceToUnitGroupDataSet", "value": {"shortDescription": [{"value": "kg NMVOC eqv.", "lang": "en"}], "type": "unit group data set", "refObjectId": "d27c25f8-fbc1-44c6-b47b-4adbae4199c6"}}, {"value": "0.5516275920112688", "module": "A1-A3"}, {"value": "0.00635063048523522", "module": "A4"}, {"value": "0.016609900084799532", "module": "A5"}, {"value": "0", "module": "B1"}, {"value": "0.13351290450303", "module": "C1"}, {"value": "0.02807147707760054", "module": "C2", "scenario": "Recycled"}, {"value": "0.02807147707760054", "module": "C2", "scenario": "Landfill"}, {"value": "0.027873762530040005", "module": "C3", "scenario": "Recycled"}, {"value": "0", "module": "C3", "scenario": "Landfill"}, {"value": "0", "module": "C4", "scenario": "Recycled"}, {"value": "0.1280763246513186", "module": "C4", "scenario": "Landfill"}, {"value": "-0.052122622504579816", "module": "D", "scenario": "Recycled"}, {"value": "0", "module": "D", "scenario": "Landfill"}]}}, {"referenceToLCIAMethodDataSet": {"shortDescription": [{"value": "Abiotic depletion potential - non-fossil resources (ADPE)", "lang": "en"}], "type": "LCIA method data set", "refObjectId": "b2ad6494-c78d-11e6-9d9d-cec0c932ce01"}, "other": {"anies": [{"name": "referenceToUnitGroupDataSet", "value": {"shortDescription": [{"value": "kg Sb eqv.", "lang": "en"}], "type": "unit group data set", "refObjectId": "54ccd2d9-a32a-4fc2-923d-f2c8c93e89d4"}}, {"value": "0.00012734626983009533", "module": "A1-A3"}, {"value": "1.4679707932717703E-05", "module": "A4"}, {"value": "1.1213384580756838E-06", "module": "A5"}, {"value": "0", "module": "B1"}, {"value": "5.07748840748972E-06", "module": "C1"}, {"value": "1.494199011615403E-05", "module": "C2", "scenario": "Recycled"}, {"value": "1.494199011615403E-05", "module": "C2", "scenario": "Landfill"}, {"value": "6.768259549200001E-06", "module": "C3", "scenario": "Recycled"}, {"value": "0", "module": "C3", "scenario": "Landfill"}, {"value": "0", "module": "C4", "scenario": "Recycled"}, {"value": "2.8482828252171264E-05", "module": "C4", "scenario": "Landfill"}, {"value": "-0.00013284667352609999", "module": "D", "scenario": "Recycled"}, {"value": "0", "module": "D", "scenario": "Landfill"}]}}, {"referenceToLCIAMethodDataSet": {"shortDescription": [{"value": "Abiotic depletion potential - fossil resources (ADPF)", "lang": "en"}], "type": "LCIA method data set", "refObjectId": "b2ad6110-c78d-11e6-9d9d-cec0c932ce01"}, "other": {"anies": [{"name": "referenceToUnitGroupDataSet", "value": {"shortDescription": [{"value": "MJ", "lang": "en"}], "type": "unit group data set", "refObjectId": "93a60a57-a3c8-11da-a746-0800200c9a66"}}, {"value": "917.3741313413508", "module": "A1-A3"}, {"value": "57.3247101934322", "module": "A4"}, {"value": "20.68165692541988", "module": "A5"}, {"value": "0", "module": "B1"}, {"value": "132.059046495382", "module": "C1"}, {"value": "97.11962897707474", "module": "C2", "scenario": "Recycled"}, {"value": "97.11962897707474", "module": "C2", "scenario": "Landfill"}, {"value": "64.36276296861061", "module": "C3", "scenario": "Recycled"}, {"value": "0", "module": "C3", "scenario": "Landfill"}, {"value": "0", "module": "C4", "scenario": "Recycled"}, {"value": "343.5247575258624", "module": "C4", "scenario": "Landfill"}, {"value": "-112.41707377541465", "module": "D", "scenario": "Recycled"}, {"value": "0", "module": "D", "scenario": "Landfill"}]}}, {"referenceToLCIAMethodDataSet": {"shortDescription": [{"value": "Water (user) deprivation potential (WDP)", "lang": "en"}], "type": "LCIA method data set", "refObjectId": "b2ad66ce-c78d-11e6-9d9d-cec0c932ce01"}, "other": {"anies": [{"name": "referenceToUnitGroupDataSet", "value": {"shortDescription": [{"value": "m^(3) world eqv.", "lang": "en"}], "type": "unit group data set", "refObjectId": "6ae2df01-888e-46c8-b17d-49fa3869b476"}}, {"value": "34.427963489861796", "module": "A1-A3"}, {"value": "0.1906337037552452", "module": "A4"}, {"value": "0.16911891853596797", "module": "A5"}, {"value": "0", "module": "B1"}, {"value": "0.206647138173278", "module": "C1"}, {"value": "0.3723523106932211", "module": "C2", "scenario": "Recycled"}, {"value": "0.3723523106932211", "module": "C2", "scenario": "Landfill"}, {"value": "0.56270955769893", "module": "C3", "scenario": "Recycled"}, {"value": "0", "module": "C3", "scenario": "Landfill"}, {"value": "0", "module": "C4", "scenario": "Recycled"}, {"value": "15.462284039744233", "module": "C4", "scenario": "Landfill"}, {"value": "25.330260120836563", "module": "D", "scenario": "Recycled"}, {"value": "0", "module": "D", "scenario": "Landfill"}]}}, {"referenceToLCIAMethodDataSet": {"shortDescription": [{"value": "Potential incidence of disease due to PM emissions (PM)", "lang": "en"}], "type": "LCIA method data set", "refObjectId": "b5c602c6-def3-11e6-bf01-fe55135034f3"}, "other": {"anies": [{"name": "referenceToUnitGroupDataSet", "value": {"shortDescription": [{"value": "disease incidence", "lang": "en"}], "type": "unit group data set", "refObjectId": "3883559b-648f-4afc-8ba2-0bd24f3affa3"}}, {"value": "5.865338838715644E-06", "module": "A1-A3"}, {"value": "2.5873609499422913E-07", "module": "A4"}, {"value": "3.344857115157377E-07", "module": "A5"}, {"value": "0", "module": "B1"}, {"value": "2.68079042007178E-06", "module": "C1"}, {"value": "7.315342639683367E-07", "module": "C2", "scenario": "Recycled"}, {"value": "7.315342639683367E-07", "module": "C2", "scenario": "Landfill"}, {"value": "5.511245011200001E-07", "module": "C3", "scenario": "Recycled"}, {"value": "0", "module": "C3", "scenario": "Landfill"}, {"value": "0", "module": "C4", "scenario": "Recycled"}, {"value": "2.329396705138004E-06", "module": "C4", "scenario": "Landfill"}, {"value": "-1.0699274387898874E-06", "module": "D", "scenario": "Recycled"}, {"value": "0", "module": "D", "scenario": "Landfill"}]}}, {"referenceToLCIAMethodDataSet": {"shortDescription": [{"value": "Potential Human exposure efficiency relative to U235 (IRP)", "lang": "en"}], "type": "LCIA method data set", "refObjectId": "b5c632be-def3-11e6-bf01-fe55135034f3"}, "other": {"anies": [{"name": "referenceToUnitGroupDataSet", "value": {"shortDescription": [{"value": "kBq U235 eq.", "lang": "en"}], "type": "unit group data set", "refObjectId": "456b05bf-1415-44a9-9993-02452f554c09"}}, {"value": "9.803698977767429", "module": "A1-A3"}, {"value": "0.2992496199351879", "module": "A4"}, {"value": "0.18381901672016376", "module": "A5"}, {"value": "0", "module": "B1"}, {"value": "0.595231370517692", "module": "C1"}, {"value": "0.45830864583442504", "module": "C2", "scenario": "Recycled"}, {"value": "0.45830864583442504", "module": "C2", "scenario": "Landfill"}, {"value": "1.7567008060673701", "module": "C3", "scenario": "Recycled"}, {"value": "0", "module": "C3", "scenario": "Landfill"}, {"value": "0", "module": "C4", "scenario": "Recycled"}, {"value": "1.5255937765619734", "module": "C4", "scenario": "Landfill"}, {"value": "-3.122463874216792", "module": "D", "scenario": "Recycled"}, {"value": "0", "module": "D", "scenario": "Landfill"}]}}, {"referenceToLCIAMethodDataSet": {"shortDescription": [{"value": "Potential Comparative Toxic Unit for ecosystems (ETP-fw)", "lang": "en"}], "type": "LCIA method data set", "refObjectId": "ee1082d1-b0f7-43ca-a1f0-21e2a4a74511"}, "other": {"anies": [{"name": "referenceToUnitGroupDataSet", "value": {"shortDescription": [{"value": "CTUe", "lang": "en"}], "type": "unit group data set", "refObjectId": "aa959ded-f1eb-4efb-9c5c-2d60be36b3e6"}}, {"value": "606.8586322730548", "module": "A1-A3"}, {"value": "46.42705965992982", "module": "A4"}, {"value": "8.06709707252943", "module": "A5"}, {"value": "0", "module": "B1"}, {"value": "36.6735102280032", "module": "C1"}, {"value": "32.84781798392806", "module": "C2", "scenario": "Recycled"}, {"value": "32.84781798392806", "module": "C2", "scenario": "Landfill"}, {"value": "33.33473223815341", "module": "C3", "scenario": "Recycled"}, {"value": "0", "module": "C3", "scenario": "Landfill"}, {"value": "0", "module": "C4", "scenario": "Recycled"}, {"value": "94.5506768170132", "module": "C4", "scenario": "Landfill"}, {"value": "-159.03545637120183", "module": "D", "scenario": "Recycled"}, {"value": "0", "module": "D", "scenario": "Landfill"}]}}, {"referenceToLCIAMethodDataSet": {"shortDescription": [{"value": "Potential Comparative Toxic Unit for humans - cancer effects (HTP-c)", "lang": "en"}], "type": "LCIA method data set", "refObjectId": "2299222a-bbd8-474f-9d4f-4dd1f18aea7c"}, "other": {"anies": [{"name": "referenceToUnitGroupDataSet", "value": {"shortDescription": [{"value": "CTUh", "lang": "en"}], "type": "unit group data set", "refObjectId": "d4c9523e-2d7e-49fd-8469-998f547d3a70"}}, {"value": "3.1926980296199744E-08", "module": "A1-A3"}, {"value": "1.5535130421784319E-09", "module": "A4"}, {"value": "3.2428760929340136E-10", "module": "A5"}, {"value": "0", "module": "B1"}, {"value": "2.98891256721161E-09", "module": "C1"}, {"value": "2.115071463109447E-09", "module": "C2", "scenario": "Recycled"}, {"value": "2.115071463109447E-09", "module": "C2", "scenario": "Landfill"}, {"value": "9.7868694888E-10", "module": "C3", "scenario": "Recycled"}, {"value": "0", "module": "C3", "scenario": "Landfill"}, {"value": "0", "module": "C4", "scenario": "Recycled"}, {"value": "5.503966333157641E-09", "module": "C4", "scenario": "Landfill"}, {"value": "-1.2369960552724295E-08", "module": "D", "scenario": "Recycled"}, {"value": "0", "module": "D", "scenario": "Landfill"}]}}, {"referenceToLCIAMethodDataSet": {"shortDescription": [{"value": "Potential Comparative Toxic Unit for humans - non-cancer effects (HTP-nc)", "lang": "en"}], "type": "LCIA method data set", "refObjectId": "3af763a5-b7a1-48c9-9cee-1f223481fcef"}, "other": {"anies": [{"name": "referenceToUnitGroupDataSet", "value": {"shortDescription": [{"value": "CTUh", "lang": "en"}], "type": "unit group data set", "refObjectId": "d4c9523e-2d7e-49fd-8469-998f547d3a70"}}, {"value": "1.5702774890413507E-06", "module": "A1-A3"}, {"value": "4.8560891953269145E-08", "module": "A4"}, {"value": "1.2448368120868261E-08", "module": "A5"}, {"value": "0", "module": "B1"}, {"value": "5.60601801217844E-08", "module": "C1"}, {"value": "8.399127804157456E-08", "module": "C2", "scenario": "Recycled"}, {"value": "8.399127804157456E-08", "module": "C2", "scenario": "Landfill"}, {"value": "2.0800507625100002E-08", "module": "C3", "scenario": "Recycled"}, {"value": "0", "module": "C3", "scenario": "Landfill"}, {"value": "0", "module": "C4", "scenario": "Recycled"}, {"value": "1.4263838991215087E-07", "module": "C4", "scenario": "Landfill"}, {"value": "-2.05355223034742E-07", "module": "D", "scenario": "Recycled"}, {"value": "0", "module": "D", "scenario": "Landfill"}]}}, {"referenceToLCIAMethodDataSet": {"shortDescription": [{"value": "Potential Soil quality index (SQP)", "lang": "en"}], "type": "LCIA method data set", "refObjectId": "b2ad6890-c78d-11e6-9d9d-cec0c932ce01"}, "other": {"anies": [{"name": "referenceToUnitGroupDataSet", "value": {"shortDescription": [{"value": "-", "lang": "en"}], "type": "unit group data set", "refObjectId": "f130951c-e67f-4f7f-8dd4-665de3974e18"}}, {"value": "1064.9722997602762", "module": "A1-A3"}, {"value": "63.937090466036345", "module": "A4"}, {"value": "5.83483751746107", "module": "A5"}, {"value": "0", "module": "B1"}, {"value": "16.8167760604904", "module": "C1"}, {"value": "109.72870096218888", "module": "C2", "scenario": "Recycled"}, {"value": "109.72870096218888", "module": "C2", "scenario": "Landfill"}, {"value": "9.622511154731072", "module": "C3", "scenario": "Recycled"}, {"value": "0", "module": "C3", "scenario": "Landfill"}, {"value": "0", "module": "C4", "scenario": "Recycled"}, {"value": "721.0096813707524", "module": "C4", "scenario": "Landfill"}, {"value": "-284.44215350589917", "module": "D", "scenario": "Recycled"}, {"value": "0", "module": "D", "scenario": "Landfill"}]}}]}, "otherAttributes": {"{http://www.indata.network/EPD/2019}epd-version": "1.2"}, "version": "1.1"}