{"processInformation": {"dataSetInformation": {"UUID": "30b730ce-ef6f-45af-97de-8cebf6aa91a9", "name": {"baseName": [{"value": "Krinner Schraubfundamente", "lang": "de"}, {"value": "KRINNER Ground Screws", "lang": "en"}], "functionalUnitFlowProperties": [{"lang": "de"}]}, "classificationInformation": {"classification": [{"class": [{"value": "Metalle", "level": 0, "classId": "4"}, {"value": "Stahl und Eisen", "level": 1, "classId": "4.1"}, {"value": "Befestigungsmittel", "level": 2, "classId": "4.1.06"}], "name": "OEKOBAU.DAT"}, {"class": [{"value": "02 Bauprodukte", "level": 0}, {"value": "Metallbauprodukte und Zubehör", "level": 1}, {"value": "Baustähle", "level": 2}], "name": "IBUCategories"}]}, "generalComment": [{"value": "Krinner Schraubfundamente sind konisch zulaufende Stahlpfhle, die drehend in den Boden eingebracht werden und zur Einleitung von axialen Zug- und Druckkrften in den Untergrund verwendet werden knnen.", "lang": "de"}, {"value": "Krinner ground screws are tapered steel piles that are inserted into the ground in a rotating manner and can be used to transfer axial tensile and compressive forces into the subsoil. \nThe ground screws partly replace solid foundations and basically ensure the load transfer of the structure into the subsoil. For example, the ground screws in the V-series consist of a 2.0-metre-long base element with a drill point and a top plate as well as any necessary extension elements. The individual sections can be coupled together by means of a plug-in connection and thus extended to the required length. Depending on the type, they have different construction lengths and diameters. The ground screws are driven into the ground to the required depth by means of an excavator, for example. \n\nThe ground screws are made of steel and are hot-dip galvanised.", "lang": "en"}]}, "quantitativeReference": {"referenceToReferenceFlow": [0]}, "time": {"referenceYear": 2023, "dataSetValidUntil": 2028, "other": {"anies": [{"name": "publicationDateOfEPD", "value": 1694390400000}]}}, "geography": {"locationOfOperationSupplyOrProduction": {"location": "DE"}}, "technology": {"technologyDescriptionAndIncludedProcesses": [{"value": "Nach der Anlieferung der Stahlrohre werden diese mit Hilfe von Sägen und Lasern auf Länge geschnitten. Das Ausgangsmaterial wird so bestellt, dass kein Abfall anfällt. Falls aufgrund von Ausschuss doch Abfall anfällt, wird dieser in Behältern gelagert und von einem Schrotthändler abgeholt, der diesen gemäß Vorschrift dem Recycling zuführt. Formgebung und Weiterverarbeitung In mehreren Arbeitsschritten, die Kalt- und Warmumformung, Brennschneiden, Stanzen beinhalten, werden die Rohre so in ihre finale, konische Form gebracht, die KRINNER Spitze geformt und die notwendigen Löcher an den Profilen angebracht. Im Anschluss werden die jeweils für das Produkt spezifischen Anschlusslösungen an die Kopfseite des Produktes halbautomatisch bzw. durch einen Schweißroboter angeschweißt. Im finalen Arbeitsschritt werden die Gewindecoils halbautomatisch auf das Profil aufgeschweißt. Korrosionsschutz Die fertigen KRINNER Schraubfundamente werden dann gemäß DIN EN ISO 1461:2009 feuerverzinkt, um beim weiteren Einsatz Korrosion zu verhindern und die Lebensdauer des Produkts zu maximieren. Qualitätsmanagement KRINNER Schraubfundamente handelt nach einem integriertem Managementsystem nach ISO 9001:2015. \nTechnische Daten: \nEs gelten die folgenden technischen Daten fr die Krinner Schraubfundamente. Die Prfnorm ist die EN 1090-2. \nDeklarierte Einheit: \nDie Deklaration bezieht sich auf die Herstellung von 1 kg Krinner Schraubfundamente als Durchschnittsprodukt verschiedener Schraubfundamente-Serien des Herstellers KRINNER Schraubfundamente GmbH fr das Jahr 2021 (ausgenommen U-, G- und K-Serie). Hierbei wurde die fakturierte Menge der verschiedenen Schraubfundamentgren bezogen auf das Betrachtungsjahr geteilt durch das Gesamtgewicht der Produkte.", "lang": "de"}, {"value": "After the steel pipes are delivered, they are cut to length using saws and lasers. The raw material is ordered so that no waste is produced. If waste does occur due to rejects, it is stored in containers and collected by a scrap dealer who recycles it according to regulations. Shaping and further processing In several work steps involving cold and hot forming, flame cutting and punching, the tubes are thus shaped into their final conical form, the Krinner tip is formed, and the necessary holes are made in the profiles. Subsequently, the connection solutions specific to the product are welded to the head side of the product semi-automatically or by a welding robot. In a final step, the thread coils are welded onto the profile semi-automatically. Corrosion protection The finished Krinner ground screws are then hot-dip galvanised in accordance with ISO 1461 to prevent corrosion during subsequent use and to maximise the life of the product. Quality management Krinner Schraubfundamente GmbH operates in accordance with an integrated management system to ISO 9001. \nTechnical data: \nThe following technical data applies to Krinner ground screws. The test standard is EN 1090-2. \nDeclared unit: \nThe Declaration refers to the production of 1 kg of Krinner ground screws as an average product of various ground screw series manufactured by KRINNER Schraubfundamente GmbH for the year 2021 (excluding the U-, G- and K-series). Here, the invoiced quantity of the various ground screw sizes related to the year under consideration was divided by the total weight of the products.", "lang": "en"}], "technologicalApplicability": [{"value": "KRINNER Schraubfundamente werden bei Gebuden und anderen gewhnlichen Tragwerken nach Eurocode 0, wie z. B.: Wohnhusern, Kindergrten, Schulen, Modulbauanlagen, Hallen, Tiny-Husern, Gartenhusern, Gewchshusern, Carports, Baumhusern, Ferienhusern, Hotels, Brogebuden, Arbeitsrumen, etc. in Holz- und Stahlstnderbauweise- bzw. Stahl-Leichtbauweise eingesetzt sowie fr Lrmschutzwnde, Hangsicherungen/-Sicherungen, Treppenanlagen, Steganlagen, Container, Masten, Schilder, E-Ladesulen, Zaunanlagen etc. Auch fr Massivbauten knnen Schraubfundamente, z.B. untersttzend unter der Bodenplatte, eingesetzt werden; je nach erforderlicher Tragfhigkeit der projektspezifischen Gegebenheiten.\n\nE- Serie\nDie Schraubfundamente der E-Serie sind optional und je nach Anwendungsgebiet mit Exzentersatz ausgestattet. Der Exzenter ermglicht die Feinjustierung fr einen perfekten, senkrechten Stand des aufzustellenden Objekts. Das System ist besonders geeignet fr die resonanz- und schwingungshemmende Montage von z. B. Rohrpfosten und Masten.\n\nF- Serie\nDie Schraubfundamente der F-Serie sind mit runden oder eckigen Flanschen ausgestattet. Die dadurch mgliche Fixierung des zu tragenden Objekts sorgt fr verbesserte Stabilitt und Sicherheit bei groen statischen Lasten.\n\nG- Serie\nDie Schraubfundamente der G-Serie sind mit einer, drei oder vier Gewindeschrauben ausgestattet. Sie eignen sich damit insbesondere fr die schnelle senkrechte und dauerhafte Montage von zum Beispiel Masten und Zaunpfosten.\n\nM- Serie \nDie Schraubfundamente der M-Serie verfgen ber ein zentriertes M-Gewinde, welches das direkte Anschrauben des zu tragenden Objekts an das Schraubfundament ermglicht. Es eignet sich damit z. B. fr Fertiggaragen und Container.\n\nU- Serie\nDie Schraubfundamente der U-Serie sind speziell abgestimmt auf die gngigen Mae von Holzbalken. Sie eignen sich insbesondere zur einfachen und schnellen Befestigung liegender und stehender Hlzer wie beispielsweise beim Carport- und Holzterrassenbau.\n\nV- Serie\nDie Schraubfundamente der V-Serie zhlen zu den verlngerbaren Schraubfundamenten. Je nach Projekt knnen die Schraubfundamente erweitert werden und wurden somit speziell fr Projekte mit hohen Lastaufnahmeanforderungen entwickelt.\n\nX- Serie \nDie Schraubfundamente der X-Serie werden fr spezielle Anwendungen nach Ma entwickelt. Je nach Anforderung werden die Fundamente passgenau und individuell gefertigt.", "lang": "de"}, {"value": "KRINNER ground screws are used for buildings and other ordinary load-bearing structures according to Eurocode 0, such as: residential buildings, kindergartens, schools, modular buildings, halls, tiny houses, garden houses, greenhouses, carports, tree houses, holiday homes, hotels, office buildings, workrooms etc., in timber and steel post-and-beam construction or lightweight steel construction, as well as for noise barriers, slope protection/securing, staircases, footbridges, containers, masts, signs, electric charging columns, fencing etc. Ground screws can also be used for solid buildings, e.g. as a support under the floor slab, depending on the required load-bearing capacity of the project-specific conditions.\n\nE- Series\nThe ground screws in the E-series are optionally equipped with an eccentric set depending on the application. The eccentric allows fine adjustment for a perfect, vertical stand of the object to be erected. The system is particularly suitable for resonance- and vibration-resistant mounting of tubular posts and masts, for example.\n\nF- Series\nThe ground screws in the F-series feature round or square flanges. The resulting fixation of the object to be supported provides improved stability and safety for large static loads.\n\nG- Series\n The ground screws in the G-series feature one, three or four threaded screws. They are therefore particularly suitable for fast vertical and permanent installation of poles and fence posts, for example.\n\nM-series \nThe ground screws in the M-series have a centred M-thread, which enables the object to be supported to be screwed directly onto the ground screw. This makes it suitable for prefabricated garages and containers, for example. \n\nU-series \nThe ground screws in the U-series are specially adapted to the common dimensions of wooden beams. They are particularly suitable for easy and fast fastening of horizontal and vertical timber in carport and wooden terrace construction, for example. \n\nV-series \nThe ground screws in the V-series are extendable ground screws. Depending on the project, these ground screws can be extended and were thus specially developed for projects with high load-bearing requirements. \n\nX-series \nThe ground screws in the X-series are customised for special applications. Depending on the requirements, the foundations are manufactured to fit precisely and individually.", "lang": "en"}]}}, "modellingAndValidation": {"LCIMethodAndAllocation": {"typeOfDataSet": "EPD", "referenceToLCAMethodDetails": [{"shortDescription": [{"value": "Baustähle.pdf", "lang": "de"}], "type": "source data set", "refObjectId": "ad81e8be-b3b5-48d0-985f-36cbc3e3af1a"}], "other": {"anies": [{"name": "subType", "value": "average dataset"}]}}, "dataSourcesTreatmentAndRepresentativeness": {"referenceToDataSource": [{"shortDescription": [{"value": "ecoinvent database (all versions)", "lang": "de"}], "type": "source data set", "refObjectId": "b497a91f-e14b-4b69-8f28-f50eb1576766"}, {"shortDescription": [{"value": "ecoinvent 3.8 database", "lang": "de"}], "type": "source data set", "refObjectId": "0f4c65c0-6210-450f-b886-82bf8dd5ace9"}], "useAdviceForDataSet": [{"value": "Gültigkeitsbereich: \nDieses Dokument ist eine Durchschnitts-EPD fr Krinner Schraubfundamente (ausgenommen U-, kleine G- und K-Serie) der Firma KRINNER Schraubfundamente GmbH, hergestellt in Deutschland. Die deklarierte Einheit bezieht sich auf die Durchschnittsproduktion von 1 kg Krinner Schaubfundamente. Die Datenerhebung erfolgte werksspezifisch mit aktuellen Jahresdaten von 2021.\nDer Deklarationsinhaber ist verantwortlich fr die zugrunde liegenden Daten und deren Verifizierung. \nSystemgrenze: \nDie kobilanz betrachtet die Systemgrenzen \"von der Wiege bis zum Werkstor mit den Modulen C1-C4 und Modul D\" und folgt dem modularen Aufbau nach EN 15804. Die kobilanz bercksichtigt folgende Module: \nA1: Herstellung der Vorprodukte (z.B. Stahlrohre, Gewindecoils, Laserteile aus Baustahl) und projektspezifische Vorkonfektionierung einzelner Komponenten\nA2: Transport zum Hersteller: Transport der Vorprodukte zum Fertigungsstandort \nA3: Herstellungsprozesse und - aufwendungen: Begutachtung und projektspezifische Kommissionerung der einzelnen Komponenten fr die verschiedenen Ausfhrungen der Krinner Schraubfundamente-Serien.\nC1: Rckbau der Schraubfundamente\nC2: Transport zur Abfallbewirtschaftung\nC3: Abfallbewirtschaftung zur Wiederverwendung, Rckgewinnung und/oder zum Recycling\nC4: Beseitigung \nD: Wiederverwendungs-, Rckgewinnungs- oder Recyclingpotenzial als Nettoflsse und Gutschriften bzw. Lasten", "lang": "de"}, {"value": "Scope: \nThis document is an average EPD for Krinner ground screws (except U-, small G- and K-series) manufactured in Germany by KRINNER Schraubfundamente GmbH. The declared unit refers to the average production of 1 kg Krinner ground screws. The data collection was carried out on a factory-specific basis with current annual data from 2021. \nThe owner of the Declaration is responsible for the data on which it is based and verification thereof. \nThe owner of the Declaration shall be liable for the underlying information and evidence; the IBU shall not be liable with respect to manufacturer information, Life Cycle Assessment data, and evidence. This EPD was drawn up in accordance with the specifications of the EN 15804+A2. This standard is referred to as EN 15804 hereinafter. \nSystem boundary: \nThe LCA considers the system boundaries 'from the cradle to the factory gate with Modules C1-C4 and Module D' and follows the modular structure according to EN 15804. The LCA takes consideration of the following modules: \n\nA1: Manufacture of preliminary products (e.g. steel tubes, thread coils, laser parts made of structural steel) and project-specific prefabrication of individual components\nA2: Transport to manufacturer: Transport of preliminary products to the manufacturing site\nA3: Manufacturing processes and expenses: Assessment and project-specific commissioning of the individual components for the various versions of the Krinner ground screw series\nC1: Deconstruction of the ground screws\nC2: Transport to waste treatment\nC3: Waste management for reuse, recovery and/or recycling\nC4: Disposal\nD: Reuse, recovery or recycling potential as net flows and credits or loads", "lang": "en"}], "other": {"anies": [{"name": "referenceToOriginalEPD", "value": {"shortDescription": {"value": "Krinner Schraubfundamente.pdf", "defaultValue": "Krinner Schraubfundamente.pdf", "lstrings": [{"lang": "de", "value": "Krinner Schraubfundamente.pdf"}]}, "type": "source data set", "uuid": {"uuid": "98d11b80-ca1e-4887-96f1-85d872d59576"}, "refObjectId": "98d11b80-ca1e-4887-96f1-85d872d59576", "resourceURLs": ["https://oekobaudat.de/OEKOBAU.DAT/resource/sources/98d11b80-ca1e-4887-96f1-85d872d59576/Krinner_Schraubfundamente_18883.pdf?version=00.02.000"]}}]}}, "validation": {"review": [{"referenceToNameOfReviewerAndInstitution": [{"shortDescription": [{"value": "Institut Bauen und Umwelt e. V.", "lang": "de"}], "type": "contact data set", "refObjectId": "d111dbec-b024-4be5-86c5-752d6eb2cf95", "uri": "../contacts/d111dbec-b024-4be5-86c5-752d6eb2cf95.xml"}], "type": "Accredited third party review"}]}, "complianceDeclarations": {"compliance": [{"referenceToComplianceSystem": {"shortDescription": [{"value": "DIN EN 15804+A2", "lang": "de"}], "type": "source data set", "refObjectId": "c0016b33-8cf7-415c-ac6e-deba0d21440d", "uri": "../sources/c0016b33-8cf7-415c-ac6e-deba0d21440d.xml"}}, {"referenceToComplianceSystem": {"shortDescription": [{"value": "ISO 14025", "lang": "de"}], "type": "source data set", "refObjectId": "4f2eb655-6e44-4874-a95a-e28f5442cd4d", "uri": "../sources/4f2eb655-6e44-4874-a95a-e28f5442cd4d.xml"}}]}}, "administrativeInformation": {"commissionerAndGoal": {"referenceToCommissioner": [{"shortDescription": [{"value": "Krinner Schraubfundamente GmbH", "lang": "de"}], "type": "contact data set", "refObjectId": "e06d33f2-126f-465d-974e-3c895cab95f7", "uri": "../contacts/e06d33f2-126f-465d-974e-3c895cab95f7.xml"}]}, "dataGenerator": {"referenceToPersonOrEntityGeneratingTheDataSet": [{"shortDescription": [{"value": "myclimate Deutschland gGmbH", "lang": "de"}], "type": "contact data set", "refObjectId": "d468648c-aeca-4188-96d2-75f5e1a561aa", "uri": "../contacts/d468648c-aeca-4188-96d2-75f5e1a561aa.xml"}]}, "dataEntryBy": {"timeStamp": 1694390400000, "referenceToDataSetFormat": [{"shortDescription": [{"value": "ILCD Format", "lang": "de"}], "type": "source data set", "refObjectId": "a97a0155-0234-4b87-b4ce-a45da52f2a40", "uri": "../sources/a97a0155-0234-4b87-b4ce-a45da52f2a40.xml"}, {"shortDescription": [{"value": "EPD-Datenformaterweiterungen v1.2", "lang": "de"}, {"value": "EPD Data Format Extensions v1.2", "lang": "en"}], "type": "source data set", "refObjectId": "a29449fd-aa2f-4de8-b5d7-4b06b43c6fde", "uri": "../sources/a29449fd-aa2f-4de8-b5d7-4b06b43c6fde.xml"}]}, "publicationAndOwnership": {"dataSetVersion": "00.08.000", "dateOfLastRevision": 1694386800000, "referenceToRegistrationAuthority": {"shortDescription": [{"value": "Institut Bauen und Umwelt e. V.", "lang": "de"}], "type": "contact data set", "refObjectId": "d111dbec-b024-4be5-86c5-752d6eb2cf95", "uri": "../contacts/d111dbec-b024-4be5-86c5-752d6eb2cf95.xml"}, "registrationNumber": "EPD-KRI-20230308-IBC1-DE", "referenceToOwnershipOfDataSet": {"shortDescription": [{"value": "Krinner Schraubfundamente GmbH", "lang": "de"}], "type": "contact data set", "refObjectId": "e06d33f2-126f-465d-974e-3c895cab95f7", "uri": "../contacts/e06d33f2-126f-465d-974e-3c895cab95f7.xml"}, "copyright": true, "licenseType": "Free of charge for all users and uses", "accessRestrictions": [{"value": "None", "lang": "en"}], "other": {"anies": [{"name": "referenceToPublisher", "value": {"shortDescription": [{"value": "Institut Bauen und Umwelt e. V.", "lang": "de"}], "type": "contact data set", "refObjectId": "d111dbec-b024-4be5-86c5-752d6eb2cf95", "uri": "../contacts/d111dbec-b024-4be5-86c5-752d6eb2cf95.xml"}}]}}}, "exchanges": {"exchange": [{"dataSetInternalID": 0, "referenceToFlowDataSet": {"shortDescription": [{"value": "Krinner Schraubfundamente (Krinner Schraubfundamente)", "lang": "de"}], "type": "flow data set", "refObjectId": "3bb1be33-ad4a-c7e3-db2b-6071f6cd9d5f", "uri": "../flows/3bb1be33-ad4a-c7e3-db2b-6071f6cd9d5f.xml"}, "meanAmount": 1.0, "referencesToDataSource": {}, "referenceFlow": true, "resolvedFlowVersion": "00.03.000", "resultingflowAmount": 1.0, "flowProperties": [{"name": [{"lang": "en", "value": "Mass"}, {"lang": "de", "value": "Masse"}], "uuid": "93a60a56-a3c8-11da-a746-0800200b9a66", "referenceFlowProperty": true, "meanValue": 1.0, "referenceUnit": "kg", "unitGroupUUID": "ad38d542-3fe9-439d-9b95-2f5f7752acaf"}], "materialProperties": [{"name": "gross density", "value": "7850.0", "unit": "kg/m^3", "unitDescription": "kilograms per cubic metre"}], "typeOfFlow": "Product flow", "classification": {"classHierarchy": "Metalle / Stahl und Eisen / Befestigungsmittel", "name": "OEKOBAU.DAT"}}, {"dataSetInternalID": 1, "referenceToFlowDataSet": {"shortDescription": [{"value": "Erneuerbare Primärenergie als Energieträger (PERE)", "lang": "de"}, {"value": "Renewable primary energy as energy carrier (PERE)", "lang": "en"}], "type": "flow data set", "refObjectId": "20f32be5-0398-4288-9b6d-accddd195317", "uri": "../flows/20f32be5-0398-4288-9b6d-accddd195317.xml"}, "exchange direction": "INPUT", "other": {"anies": [{"name": "referenceToUnitGroupDataSet", "value": {"shortDescription": [{"value": "MJ", "lang": "de"}], "type": "unit group data set", "refObjectId": "93a60a57-a3c8-11da-a746-0800200c9a66", "uri": "../unitgroups/93a60a57-a3c8-11da-a746-0800200c9a66.xml"}}, {"value": "3.2844164307", "module": "A1-A3"}, {"value": "0", "module": "C1"}, {"value": "0.00107107643", "module": "C2"}, {"value": "0.000633701612", "module": "C3"}, {"value": "0", "module": "C4"}, {"value": "-1.60297897", "module": "D"}]}, "resolvedFlowVersion": "38.00.000", "flowProperties": [], "typeOfFlow": "Other flow", "classification": {"classHierarchy": "Quantities", "name": "GaBiCategories"}}, {"dataSetInternalID": 2, "referenceToFlowDataSet": {"shortDescription": [{"value": "Erneuerbare Primärenergie zur stofflichen Nutzung (PERM)", "lang": "de"}, {"value": "Renewable primary energy resources as material utilization (PERM)", "lang": "en"}], "type": "flow data set", "refObjectId": "fb3ec0de-548d-4508-aea5-00b73bf6f702", "uri": "../flows/fb3ec0de-548d-4508-aea5-00b73bf6f702.xml"}, "exchange direction": "INPUT", "other": {"anies": [{"name": "referenceToUnitGroupDataSet", "value": {"shortDescription": [{"value": "MJ", "lang": "de"}], "type": "unit group data set", "refObjectId": "93a60a57-a3c8-11da-a746-0800200c9a66", "uri": "../unitgroups/93a60a57-a3c8-11da-a746-0800200c9a66.xml"}}, {"value": "0", "module": "A1-A3"}, {"value": "0", "module": "C1"}, {"value": "0", "module": "C2"}, {"value": "0", "module": "C3"}, {"value": "0", "module": "C4"}, {"value": "0", "module": "D"}]}, "resolvedFlowVersion": "38.00.000", "flowProperties": [], "typeOfFlow": "Other flow", "classification": {"classHierarchy": "Quantities", "name": "GaBiCategories"}}, {"dataSetInternalID": 3, "referenceToFlowDataSet": {"shortDescription": [{"value": "Total erneuerbare Primärenergie (PERT)", "lang": "de"}, {"value": "Total use of renewable primary energy resources (PERT)", "lang": "en"}], "type": "flow data set", "refObjectId": "53f97275-fa8a-4cdd-9024-65936002acd0", "uri": "../flows/53f97275-fa8a-4cdd-9024-65936002acd0.xml"}, "exchange direction": "INPUT", "other": {"anies": [{"name": "referenceToUnitGroupDataSet", "value": {"shortDescription": [{"value": "MJ", "lang": "de"}], "type": "unit group data set", "refObjectId": "93a60a57-a3c8-11da-a746-0800200c9a66", "uri": "../unitgroups/93a60a57-a3c8-11da-a746-0800200c9a66.xml"}}, {"value": "3.2844164307", "module": "A1-A3"}, {"value": "0", "module": "C1"}, {"value": "0.00107107643", "module": "C2"}, {"value": "0.000633701612", "module": "C3"}, {"value": "0", "module": "C4"}, {"value": "-1.60297897", "module": "D"}]}, "resolvedFlowVersion": "38.00.000", "flowProperties": [], "typeOfFlow": "Other flow", "classification": {"classHierarchy": "Quantities / Environmental quantities / EPD EN 15804 / LCI indicators", "name": "GaBiCategories"}}, {"dataSetInternalID": 4, "referenceToFlowDataSet": {"shortDescription": [{"value": "Nicht-erneuerbare Primärenergie als Energieträger (PENRE)", "lang": "de"}, {"value": "Non renewable primary energy as energy carrier (PENRE)", "lang": "en"}], "type": "flow data set", "refObjectId": "ac857178-2b45-46ec-892a-a9a4332f0372", "uri": "../flows/ac857178-2b45-46ec-892a-a9a4332f0372.xml"}, "exchange direction": "INPUT", "other": {"anies": [{"name": "referenceToUnitGroupDataSet", "value": {"shortDescription": [{"value": "MJ", "lang": "de"}], "type": "unit group data set", "refObjectId": "93a60a57-a3c8-11da-a746-0800200c9a66", "uri": "../unitgroups/93a60a57-a3c8-11da-a746-0800200c9a66.xml"}}, {"value": "27.726611341131", "module": "A1-A3"}, {"value": "0", "module": "C1"}, {"value": "0.0893549898165", "module": "C2"}, {"value": "0.058500878156", "module": "C3"}, {"value": "0", "module": "C4"}, {"value": "-16.9791187704", "module": "D"}]}, "resolvedFlowVersion": "38.00.000", "flowProperties": [], "typeOfFlow": "Other flow", "classification": {"classHierarchy": "Quantities", "name": "GaBiCategories"}}, {"dataSetInternalID": 5, "referenceToFlowDataSet": {"shortDescription": [{"value": "Nicht-erneuerbare Primärenergie zur stofflichen Nutzung (PENRM)", "lang": "de"}, {"value": "Non renewable primary energy as material utilization (PENRM)", "lang": "en"}], "type": "flow data set", "refObjectId": "1421caa0-679d-4bf4-b282-0eb850ccae27", "uri": "../flows/1421caa0-679d-4bf4-b282-0eb850ccae27.xml"}, "exchange direction": "INPUT", "other": {"anies": [{"name": "referenceToUnitGroupDataSet", "value": {"shortDescription": [{"value": "MJ", "lang": "de"}], "type": "unit group data set", "refObjectId": "93a60a57-a3c8-11da-a746-0800200c9a66", "uri": "../unitgroups/93a60a57-a3c8-11da-a746-0800200c9a66.xml"}}, {"value": "0", "module": "A1-A3"}, {"value": "0", "module": "C1"}, {"value": "0", "module": "C2"}, {"value": "0", "module": "C3"}, {"value": "0", "module": "C4"}, {"value": "0", "module": "D"}]}, "resolvedFlowVersion": "38.00.000", "flowProperties": [], "typeOfFlow": "Other flow", "classification": {"classHierarchy": "Quantities", "name": "GaBiCategories"}}, {"dataSetInternalID": 6, "referenceToFlowDataSet": {"shortDescription": [{"value": "Total nicht erneuerbare Primärenergie (PENRT)", "lang": "de"}, {"value": "Total use of non renewable primary energy resources (PENRT)", "lang": "en"}], "type": "flow data set", "refObjectId": "06159210-646b-4c8d-8583-da9b3b95a6c1", "uri": "../flows/06159210-646b-4c8d-8583-da9b3b95a6c1.xml"}, "exchange direction": "INPUT", "other": {"anies": [{"name": "referenceToUnitGroupDataSet", "value": {"shortDescription": [{"value": "MJ", "lang": "de"}], "type": "unit group data set", "refObjectId": "93a60a57-a3c8-11da-a746-0800200c9a66", "uri": "../unitgroups/93a60a57-a3c8-11da-a746-0800200c9a66.xml"}}, {"value": "27.726611341131", "module": "A1-A3"}, {"value": "0", "module": "C1"}, {"value": "0.0893549898165", "module": "C2"}, {"value": "0.058500878156", "module": "C3"}, {"value": "0", "module": "C4"}, {"value": "-16.9791187704", "module": "D"}]}, "resolvedFlowVersion": "38.00.000", "flowProperties": [], "typeOfFlow": "Other flow", "classification": {"classHierarchy": "Quantities / Environmental quantities / EPD EN 15804 / LCI indicators", "name": "GaBiCategories"}}, {"dataSetInternalID": 7, "referenceToFlowDataSet": {"shortDescription": [{"value": "Einsatz von Sekundärstoffen (SM)", "lang": "de"}, {"value": "Use of secondary material (SM)", "lang": "en"}], "type": "flow data set", "refObjectId": "c6a1f35f-2d09-4f54-8dfb-97e502e1ce92", "uri": "../flows/c6a1f35f-2d09-4f54-8dfb-97e502e1ce92.xml"}, "exchange direction": "INPUT", "other": {"anies": [{"name": "referenceToUnitGroupDataSet", "value": {"shortDescription": [{"value": "kg", "lang": "de"}], "type": "unit group data set", "refObjectId": "ad38d542-3fe9-439d-9b95-2f5f7752acaf", "uri": "../unitgroups/ad38d542-3fe9-439d-9b95-2f5f7752acaf.xml"}}, {"value": "0.257892345", "module": "A1-A3"}, {"value": "0", "module": "C1"}, {"value": "0", "module": "C2"}, {"value": "0", "module": "C3"}, {"value": "0", "module": "C4"}, {"value": "0.665", "module": "D"}]}, "resolvedFlowVersion": "38.00.000", "flowProperties": [], "typeOfFlow": "Other flow", "classification": {"classHierarchy": "Quantities / Environmental quantities / EPD EN 15804 / LCI indicators", "name": "GaBiCategories"}}, {"dataSetInternalID": 8, "referenceToFlowDataSet": {"shortDescription": [{"value": "Erneuerbare Sekundärbrennstoffe (RSF)", "lang": "de"}, {"value": "Use of renewable secondary fuels (RSF)", "lang": "en"}], "type": "flow data set", "refObjectId": "64333088-a55f-4aa2-9a31-c10b07816787", "uri": "../flows/64333088-a55f-4aa2-9a31-c10b07816787.xml"}, "exchange direction": "INPUT", "other": {"anies": [{"name": "referenceToUnitGroupDataSet", "value": {"shortDescription": [{"value": "MJ", "lang": "de"}], "type": "unit group data set", "refObjectId": "93a60a57-a3c8-11da-a746-0800200c9a66", "uri": "../unitgroups/93a60a57-a3c8-11da-a746-0800200c9a66.xml"}}, {"value": "0", "module": "A1-A3"}, {"value": "0", "module": "C1"}, {"value": "0", "module": "C2"}, {"value": "0", "module": "C3"}, {"value": "0", "module": "C4"}, {"value": "0", "module": "D"}]}, "resolvedFlowVersion": "38.00.000", "flowProperties": [], "typeOfFlow": "Other flow", "classification": {"classHierarchy": "Quantities / Environmental quantities / EPD EN 15804 / LCI indicators", "name": "GaBiCategories"}}, {"dataSetInternalID": 9, "referenceToFlowDataSet": {"shortDescription": [{"value": "Nicht erneuerbare Sekundärbrennstoffe (NRSF)", "lang": "de"}, {"value": "Use of non renewable secondary fuels (NRSF)", "lang": "en"}], "type": "flow data set", "refObjectId": "89def144-d39a-4287-b86f-efde453ddcb2", "uri": "../flows/89def144-d39a-4287-b86f-efde453ddcb2.xml"}, "exchange direction": "INPUT", "other": {"anies": [{"name": "referenceToUnitGroupDataSet", "value": {"shortDescription": [{"value": "MJ", "lang": "de"}], "type": "unit group data set", "refObjectId": "93a60a57-a3c8-11da-a746-0800200c9a66", "uri": "../unitgroups/93a60a57-a3c8-11da-a746-0800200c9a66.xml"}}, {"value": "0", "module": "A1-A3"}, {"value": "0", "module": "C1"}, {"value": "0", "module": "C2"}, {"value": "0", "module": "C3"}, {"value": "0", "module": "C4"}, {"value": "0", "module": "D"}]}, "resolvedFlowVersion": "38.00.000", "flowProperties": [], "typeOfFlow": "Other flow", "classification": {"classHierarchy": "Quantities / Environmental quantities / EPD EN 15804 / LCI indicators", "name": "GaBiCategories"}}, {"dataSetInternalID": 10, "referenceToFlowDataSet": {"shortDescription": [{"value": "Einsatz von Süßwasserressourcen (FW)", "lang": "de"}, {"value": "Use of net fresh water (FW)", "lang": "en"}], "type": "flow data set", "refObjectId": "3cf952c8-f3a4-461d-8c96-96456ca62246", "uri": "../flows/3cf952c8-f3a4-461d-8c96-96456ca62246.xml"}, "exchange direction": "INPUT", "other": {"anies": [{"name": "referenceToUnitGroupDataSet", "value": {"shortDescription": [{"value": "m^3", "lang": "de"}], "type": "unit group data set", "refObjectId": "cd950537-0a98-4044-9ba7-9f9a68d0a504", "uri": "../unitgroups/cd950537-0a98-4044-9ba7-9f9a68d0a504.xml"}}, {"value": "0.035466514577", "module": "A1-A3"}, {"value": "0", "module": "C1"}, {"value": "1.0011332E-05", "module": "C2"}, {"value": "4.6666063E-05", "module": "C3"}, {"value": "0", "module": "C4"}, {"value": "-0.011706551", "module": "D"}]}, "resolvedFlowVersion": "38.00.000", "flowProperties": [], "typeOfFlow": "Other flow", "classification": {"classHierarchy": "Quantities / Environmental quantities / EPD EN 15804 / LCI indicators", "name": "GaBiCategories"}}, {"dataSetInternalID": 11, "referenceToFlowDataSet": {"shortDescription": [{"value": "Gefährlicher Abfall zur Deponie (HWD)", "lang": "de"}, {"value": "Hazardous waste disposed (HWD)", "lang": "en"}], "type": "flow data set", "refObjectId": "430f9e0f-59b2-46a0-8e0d-55e0e84948fc", "uri": "../flows/430f9e0f-59b2-46a0-8e0d-55e0e84948fc.xml"}, "exchange direction": "OUTPUT", "other": {"anies": [{"name": "referenceToUnitGroupDataSet", "value": {"shortDescription": [{"value": "kg", "lang": "de"}], "type": "unit group data set", "refObjectId": "ad38d542-3fe9-439d-9b95-2f5f7752acaf", "uri": "../unitgroups/ad38d542-3fe9-439d-9b95-2f5f7752acaf.xml"}}, {"value": "0.0003841360177", "module": "A1-A3"}, {"value": "0", "module": "C1"}, {"value": "2.0366088E-07", "module": "C2"}, {"value": "9.7594864E-08", "module": "C3"}, {"value": "0", "module": "C4"}, {"value": "-0.00034131807", "module": "D"}]}, "resolvedFlowVersion": "38.00.000", "flowProperties": [], "typeOfFlow": "Other flow", "classification": {"classHierarchy": "Quantities / Environmental quantities / EPD EN 15804 / LCI indicators", "name": "GaBiCategories"}}, {"dataSetInternalID": 12, "referenceToFlowDataSet": {"shortDescription": [{"value": "Entsorgter nicht gefährlicher Abfall (NHWD)", "lang": "de"}, {"value": "Non hazardous waste disposed (NHWD)", "lang": "en"}], "type": "flow data set", "refObjectId": "b29ef66b-e286-4afa-949f-62f1a7b4d7fa", "uri": "../flows/b29ef66b-e286-4afa-949f-62f1a7b4d7fa.xml"}, "exchange direction": "OUTPUT", "other": {"anies": [{"name": "referenceToUnitGroupDataSet", "value": {"shortDescription": [{"value": "kg", "lang": "de"}], "type": "unit group data set", "refObjectId": "ad38d542-3fe9-439d-9b95-2f5f7752acaf", "uri": "../unitgroups/ad38d542-3fe9-439d-9b95-2f5f7752acaf.xml"}}, {"value": "0", "module": "A1-A3"}, {"value": "0", "module": "C1"}, {"value": "0", "module": "C2"}, {"value": "0", "module": "C3"}, {"value": "0", "module": "C4"}, {"value": "0", "module": "D"}]}, "resolvedFlowVersion": "38.00.000", "flowProperties": [], "typeOfFlow": "Other flow", "classification": {"classHierarchy": "Quantities / Environmental quantities / EPD EN 15804 / LCI indicators", "name": "GaBiCategories"}}, {"dataSetInternalID": 13, "referenceToFlowDataSet": {"shortDescription": [{"value": "Entsorgter radioaktiver Abfall (RWD)", "lang": "de"}, {"value": "Radioactive waste disposed (RWD)", "lang": "en"}], "type": "flow data set", "refObjectId": "3449546e-52ad-4b39-b809-9fb77cea8ff6", "uri": "../flows/3449546e-52ad-4b39-b809-9fb77cea8ff6.xml"}, "exchange direction": "OUTPUT", "other": {"anies": [{"name": "referenceToUnitGroupDataSet", "value": {"shortDescription": [{"value": "kg", "lang": "de"}], "type": "unit group data set", "refObjectId": "ad38d542-3fe9-439d-9b95-2f5f7752acaf", "uri": "../unitgroups/ad38d542-3fe9-439d-9b95-2f5f7752acaf.xml"}}, {"value": "6.29865657E-05", "module": "A1-A3"}, {"value": "0", "module": "C1"}, {"value": "5.6976276E-07", "module": "C2"}, {"value": "3.5860392E-07", "module": "C3"}, {"value": "0", "module": "C4"}, {"value": "-3.0401439E-05", "module": "D"}]}, "resolvedFlowVersion": "38.00.000", "flowProperties": [], "typeOfFlow": "Other flow", "classification": {"classHierarchy": "Quantities / Environmental quantities / EPD EN 15804 / LCI indicators", "name": "GaBiCategories"}}, {"dataSetInternalID": 14, "referenceToFlowDataSet": {"shortDescription": [{"value": "Komponenten für die Wiederverwendung (CRU)", "lang": "de"}, {"value": "Components for re-use (CRU)", "lang": "en"}], "type": "flow data set", "refObjectId": "a2b32f97-3fc7-4af2-b209-525bc6426f33", "uri": "../flows/a2b32f97-3fc7-4af2-b209-525bc6426f33.xml"}, "exchange direction": "OUTPUT", "other": {"anies": [{"name": "referenceToUnitGroupDataSet", "value": {"shortDescription": [{"value": "kg", "lang": "de"}], "type": "unit group data set", "refObjectId": "ad38d542-3fe9-439d-9b95-2f5f7752acaf", "uri": "../unitgroups/ad38d542-3fe9-439d-9b95-2f5f7752acaf.xml"}}, {"value": "0", "module": "A1-A3"}, {"value": "0", "module": "C1"}, {"value": "0", "module": "C2"}, {"value": "0", "module": "C3"}, {"value": "0", "module": "C4"}, {"value": "0", "module": "D"}]}, "resolvedFlowVersion": "38.00.000", "flowProperties": [], "typeOfFlow": "Other flow", "classification": {"classHierarchy": "Quantities / Environmental quantities / EPD EN 15804 / LCI indicators", "name": "GaBiCategories"}}, {"dataSetInternalID": 15, "referenceToFlowDataSet": {"shortDescription": [{"value": "Stoffe zum Recycling (MFR)", "lang": "de"}, {"value": "Materials for recycling (MFR)", "lang": "en"}], "type": "flow data set", "refObjectId": "d7fe48a5-4103-49c8-9aae-b0b5dfdbd6ae", "uri": "../flows/d7fe48a5-4103-49c8-9aae-b0b5dfdbd6ae.xml"}, "exchange direction": "OUTPUT", "other": {"anies": [{"name": "referenceToUnitGroupDataSet", "value": {"shortDescription": [{"value": "kg", "lang": "de"}], "type": "unit group data set", "refObjectId": "ad38d542-3fe9-439d-9b95-2f5f7752acaf", "uri": "../unitgroups/ad38d542-3fe9-439d-9b95-2f5f7752acaf.xml"}}, {"value": "0", "module": "A1-A3"}, {"value": "0", "module": "C1"}, {"value": "0", "module": "C2"}, {"value": "0.903", "module": "C3"}, {"value": "0", "module": "C4"}, {"value": "0", "module": "D"}]}, "resolvedFlowVersion": "38.00.000", "flowProperties": [], "typeOfFlow": "Other flow", "classification": {"classHierarchy": "Quantities / Environmental quantities / EPD EN 15804 / LCI indicators", "name": "GaBiCategories"}}, {"dataSetInternalID": 16, "referenceToFlowDataSet": {"shortDescription": [{"value": "Stoffe für die Energierückgewinnung (MER)", "lang": "de"}, {"value": "Materials for energy recovery (MER)", "lang": "en"}], "type": "flow data set", "refObjectId": "59a9181c-3aaf-46ee-8b13-2b3723b6e447", "uri": "../flows/59a9181c-3aaf-46ee-8b13-2b3723b6e447.xml"}, "exchange direction": "OUTPUT", "other": {"anies": [{"name": "referenceToUnitGroupDataSet", "value": {"shortDescription": [{"value": "kg", "lang": "de"}], "type": "unit group data set", "refObjectId": "ad38d542-3fe9-439d-9b95-2f5f7752acaf", "uri": "../unitgroups/ad38d542-3fe9-439d-9b95-2f5f7752acaf.xml"}}, {"value": "0", "module": "A1-A3"}, {"value": "0", "module": "C1"}, {"value": "0", "module": "C2"}, {"value": "0", "module": "C3"}, {"value": "0", "module": "C4"}, {"value": "0", "module": "D"}]}, "resolvedFlowVersion": "38.00.000", "flowProperties": [], "typeOfFlow": "Other flow", "classification": {"classHierarchy": "Quantities / Environmental quantities / EPD EN 15804 / LCI indicators", "name": "GaBiCategories"}}, {"dataSetInternalID": 17, "referenceToFlowDataSet": {"shortDescription": [{"value": "Exportierte elektrische Energie (EEE)", "lang": "de"}, {"value": "Exported electrical energy (EEE)", "lang": "en"}], "type": "flow data set", "refObjectId": "4da0c987-2b76-40d6-9e9e-82a017aaaf29", "uri": "../flows/4da0c987-2b76-40d6-9e9e-82a017aaaf29.xml"}, "exchange direction": "OUTPUT", "other": {"anies": [{"name": "referenceToUnitGroupDataSet", "value": {"shortDescription": [{"value": "MJ", "lang": "de"}], "type": "unit group data set", "refObjectId": "93a60a57-a3c8-11da-a746-0800200c9a66", "uri": "../unitgroups/93a60a57-a3c8-11da-a746-0800200c9a66.xml"}}, {"value": "0", "module": "A1-A3"}, {"value": "0", "module": "C1"}, {"value": "0", "module": "C2"}, {"value": "0", "module": "C3"}, {"value": "0", "module": "C4"}, {"value": "0", "module": "D"}]}, "resolvedFlowVersion": "38.00.000", "flowProperties": [], "typeOfFlow": "Other flow", "classification": {"classHierarchy": "Quantities / Environmental quantities / EPD EN 15804 / LCI indicators", "name": "GaBiCategories"}}, {"dataSetInternalID": 18, "referenceToFlowDataSet": {"shortDescription": [{"value": "Exportierte thermische Energie (EET)", "lang": "de"}, {"value": "Exported thermal energy (EET)", "lang": "en"}], "type": "flow data set", "refObjectId": "98daf38a-7a79-46d3-9a37-2b7bd0955810", "uri": "../flows/98daf38a-7a79-46d3-9a37-2b7bd0955810.xml"}, "exchange direction": "OUTPUT", "other": {"anies": [{"name": "referenceToUnitGroupDataSet", "value": {"shortDescription": [{"value": "MJ", "lang": "de"}], "type": "unit group data set", "refObjectId": "93a60a57-a3c8-11da-a746-0800200c9a66", "uri": "../unitgroups/93a60a57-a3c8-11da-a746-0800200c9a66.xml"}}, {"value": "0", "module": "A1-A3"}, {"value": "0", "module": "C1"}, {"value": "0", "module": "C2"}, {"value": "0", "module": "C3"}, {"value": "0", "module": "C4"}, {"value": "0", "module": "D"}]}, "resolvedFlowVersion": "38.00.000", "flowProperties": [], "typeOfFlow": "Other flow", "classification": {"classHierarchy": "Quantities / Environmental quantities / EPD EN 15804 / LCI indicators", "name": "GaBiCategories"}}]}, "LCIAResults": {"LCIAResult": [{"referenceToLCIAMethodDataSet": {"shortDescription": [{"value": "Globales Erwärmungspotenzial total (GWP-total)", "lang": "de"}, {"value": "Global Warming Potential total (GWP-total)", "lang": "en"}], "type": "LCIA method data set", "refObjectId": "6a37f984-a4b3-458a-a20a-64418c145fa2", "uri": "../lciamethods/6a37f984-a4b3-458a-a20a-64418c145fa2.xml"}, "other": {"anies": [{"name": "referenceToUnitGroupDataSet", "value": {"shortDescription": [{"value": "kg CO_(2)-Äq.", "lang": "de"}], "type": "unit group data set", "refObjectId": "1ebf3012-d0db-4de2-aefd-ef30cedb0be1", "uri": "../unitgroups/1ebf3012-d0db-4de2-aefd-ef30cedb0be1.xml"}}, {"value": "2.394654641", "module": "A1-A3"}, {"value": "0", "module": "C1"}, {"value": "0.0054030376", "module": "C2"}, {"value": "0.0023972115", "module": "C3"}, {"value": "0", "module": "C4"}, {"value": "-1.5707892", "module": "D"}]}}, {"referenceToLCIAMethodDataSet": {"shortDescription": [{"value": "Globales Erwärmungspotenzial fossil (GWP-fossil)", "lang": "de"}, {"value": "Global Warming Potential fossil fuels (GWP-fossil)", "lang": "en"}], "type": "LCIA method data set", "refObjectId": "5f635281-343e-44fb-83df-1971b155e6b6", "uri": "../lciamethods/5f635281-343e-44fb-83df-1971b155e6b6.xml"}, "other": {"anies": [{"name": "referenceToUnitGroupDataSet", "value": {"shortDescription": [{"value": "kg CO_(2)-Äq.", "lang": "de"}], "type": "unit group data set", "refObjectId": "1ebf3012-d0db-4de2-aefd-ef30cedb0be1", "uri": "../unitgroups/1ebf3012-d0db-4de2-aefd-ef30cedb0be1.xml"}}, {"value": "2.377629555", "module": "A1-A3"}, {"value": "0", "module": "C1"}, {"value": "0.0053991966", "module": "C2"}, {"value": "0.0023887697", "module": "C3"}, {"value": "0", "module": "C4"}, {"value": "-1.5676897", "module": "D"}]}}, {"referenceToLCIAMethodDataSet": {"shortDescription": [{"value": "Globales Erwärmungspotenzial biogen (GWP-biogenic)", "lang": "de"}, {"value": "Global Warming Potential biogenic (GWP-biogenic)", "lang": "en"}], "type": "LCIA method data set", "refObjectId": "2356e1ab-0185-4db5-86e5-16de51c7485c", "uri": "../lciamethods/2356e1ab-0185-4db5-86e5-16de51c7485c.xml"}, "other": {"anies": [{"name": "referenceToUnitGroupDataSet", "value": {"shortDescription": [{"value": "kg CO_(2)-Äq.", "lang": "de"}], "type": "unit group data set", "refObjectId": "1ebf3012-d0db-4de2-aefd-ef30cedb0be1", "uri": "../unitgroups/1ebf3012-d0db-4de2-aefd-ef30cedb0be1.xml"}}, {"value": "0.005070944995", "module": "A1-A3"}, {"value": "0", "module": "C1"}, {"value": "1.8997352E-06", "module": "C2"}, {"value": "1.2751674E-06", "module": "C3"}, {"value": "0", "module": "C4"}, {"value": "-0.001930186", "module": "D"}]}}, {"referenceToLCIAMethodDataSet": {"shortDescription": [{"value": "Globales Erwärmungspotenzial luluc (GWP-luluc)", "lang": "de"}, {"value": "Global Warming Potential luluc (GWP-luluc)", "lang": "en"}], "type": "LCIA method data set", "refObjectId": "4331bbdb-978a-490d-8707-eeb047f01a55", "uri": "../lciamethods/4331bbdb-978a-490d-8707-eeb047f01a55.xml"}, "other": {"anies": [{"name": "referenceToUnitGroupDataSet", "value": {"shortDescription": [{"value": "kg CO_(2)-Äq.", "lang": "de"}], "type": "unit group data set", "refObjectId": "1ebf3012-d0db-4de2-aefd-ef30cedb0be1", "uri": "../unitgroups/1ebf3012-d0db-4de2-aefd-ef30cedb0be1.xml"}}, {"value": "0.011953894001", "module": "A1-A3"}, {"value": "0", "module": "C1"}, {"value": "1.9412342E-06", "module": "C2"}, {"value": "7.1665792E-06", "module": "C3"}, {"value": "0", "module": "C4"}, {"value": "-0.001169257", "module": "D"}]}}, {"referenceToLCIAMethodDataSet": {"shortDescription": [{"value": "Abbau Potential der stratosphärischen Ozonschicht (ODP)", "lang": "de"}, {"value": "Depletion potential of the stratospheric ozone layer (ODP)", "lang": "en"}], "type": "LCIA method data set", "refObjectId": "b5c629d6-def3-11e6-bf01-fe55135034f3", "uri": "../lciamethods/b5c629d6-def3-11e6-bf01-fe55135034f3.xml"}, "other": {"anies": [{"name": "referenceToUnitGroupDataSet", "value": {"shortDescription": [{"value": "kg CFC11-Äq.", "lang": "de"}], "type": "unit group data set", "refObjectId": "d9e957c9-7309-4474-bf3a-7777df6c4e5b", "uri": "../unitgroups/d9e957c9-7309-4474-bf3a-7777df6c4e5b.xml"}}, {"value": "1.351591324E-07", "module": "A1-A3"}, {"value": "0", "module": "C1"}, {"value": "1.2894527E-09", "module": "C2"}, {"value": "7.8070544E-10", "module": "C3"}, {"value": "0", "module": "C4"}, {"value": "-7.0510595E-08", "module": "D"}]}}, {"referenceToLCIAMethodDataSet": {"shortDescription": [{"value": "Versauerungspotenzial von Boden und Wasser (AP)", "lang": "de"}, {"value": "Acidification potential of land and water (AP)", "lang": "en"}], "type": "LCIA method data set", "refObjectId": "b5c611c6-def3-11e6-bf01-fe55135034f3", "uri": "../lciamethods/b5c611c6-def3-11e6-bf01-fe55135034f3.xml"}, "other": {"anies": [{"name": "referenceToUnitGroupDataSet", "value": {"shortDescription": [{"value": "mol H^(+)-Äq.", "lang": "de"}], "type": "unit group data set", "refObjectId": "42e089ac-92bf-4bf2-8ca1-5fc40d18f2ed", "uri": "../unitgroups/42e089ac-92bf-4bf2-8ca1-5fc40d18f2ed.xml"}}, {"value": "0.0110371747", "module": "A1-A3"}, {"value": "0", "module": "C1"}, {"value": "2.2538161E-05", "module": "C2"}, {"value": "1.9595269E-05", "module": "C3"}, {"value": "0", "module": "C4"}, {"value": "-0.0071999817", "module": "D"}]}}, {"referenceToLCIAMethodDataSet": {"shortDescription": [{"value": "Eutrophierungspotenzial Süßwasser (EP-freshwater)", "lang": "de"}, {"value": "Eutrophication potential aquatic freshwater (EP-freshwater)", "lang": "en"}], "type": "LCIA method data set", "refObjectId": "b53ec18f-7377-4ad3-86eb-cc3f4f276b2b", "uri": "../lciamethods/b53ec18f-7377-4ad3-86eb-cc3f4f276b2b.xml"}, "other": {"anies": [{"name": "referenceToUnitGroupDataSet", "value": {"shortDescription": [{"value": "kg P-Äq.", "lang": "de"}], "type": "unit group data set", "refObjectId": "0429039d-a61d-4590-ba67-aa4a20a810a1", "uri": "../unitgroups/0429039d-a61d-4590-ba67-aa4a20a810a1.xml"}}, {"value": "0.0011249250802", "module": "A1-A3"}, {"value": "0", "module": "C1"}, {"value": "3.3619355E-07", "module": "C2"}, {"value": "2.502737E-07", "module": "C3"}, {"value": "0", "module": "C4"}, {"value": "-0.00080730434", "module": "D"}]}}, {"referenceToLCIAMethodDataSet": {"shortDescription": [{"value": "Eutrophierungspotenzial Salzwasser (EP-marine)", "lang": "de"}, {"value": "Eutrophication potential aquatic marine (EP-marine)", "lang": "en"}], "type": "LCIA method data set", "refObjectId": "b5c619fa-def3-11e6-bf01-fe55135034f3", "uri": "../lciamethods/b5c619fa-def3-11e6-bf01-fe55135034f3.xml"}, "other": {"anies": [{"name": "referenceToUnitGroupDataSet", "value": {"shortDescription": [{"value": "kg N-Äq.", "lang": "de"}], "type": "unit group data set", "refObjectId": "d05bb823-ecdf-4686-8c40-bf1d9257859f", "uri": "../unitgroups/d05bb823-ecdf-4686-8c40-bf1d9257859f.xml"}}, {"value": "0.002581020677", "module": "A1-A3"}, {"value": "0", "module": "C1"}, {"value": "6.8732906E-06", "module": "C2"}, {"value": "6.9069114E-06", "module": "C3"}, {"value": "0", "module": "C4"}, {"value": "-0.0015737473", "module": "D"}]}}, {"referenceToLCIAMethodDataSet": {"shortDescription": [{"value": "Eutrophierungspotenzial Land (EP-terrestrial)", "lang": "de"}, {"value": "Eutrophication potential terrestrial (EP-terrestrial)", "lang": "en"}], "type": "LCIA method data set", "refObjectId": "b5c614d2-def3-11e6-bf01-fe55135034f3", "uri": "../lciamethods/b5c614d2-def3-11e6-bf01-fe55135034f3.xml"}, "other": {"anies": [{"name": "referenceToUnitGroupDataSet", "value": {"shortDescription": [{"value": "mol N-Äq.", "lang": "de"}], "type": "unit group data set", "refObjectId": "71b4d617-0ec9-4d3f-b65e-e438940c2401", "uri": "../unitgroups/71b4d617-0ec9-4d3f-b65e-e438940c2401.xml"}}, {"value": "0.02521920504", "module": "A1-A3"}, {"value": "0", "module": "C1"}, {"value": "7.5154597E-05", "module": "C2"}, {"value": "7.5289135E-05", "module": "C3"}, {"value": "0", "module": "C4"}, {"value": "-0.016453267", "module": "D"}]}}, {"referenceToLCIAMethodDataSet": {"shortDescription": [{"value": "Bildungspotential für troposphärisches Ozon (POCP)", "lang": "de"}, {"value": "Formation potential of tropospheric ozone photochemical oxidants (POCP)", "lang": "en"}], "type": "LCIA method data set", "refObjectId": "b5c610fe-def3-11e6-bf01-fe55135034f3", "uri": "../lciamethods/b5c610fe-def3-11e6-bf01-fe55135034f3.xml"}, "other": {"anies": [{"name": "referenceToUnitGroupDataSet", "value": {"shortDescription": [{"value": "kg NMVOC-Äq.", "lang": "de"}], "type": "unit group data set", "refObjectId": "d27c25f8-fbc1-44c6-b47b-4adbae4199c6", "uri": "../unitgroups/d27c25f8-fbc1-44c6-b47b-4adbae4199c6.xml"}}, {"value": "0.01059550179", "module": "A1-A3"}, {"value": "0", "module": "C1"}, {"value": "2.4186186E-05", "module": "C2"}, {"value": "2.1781863E-05", "module": "C3"}, {"value": "0", "module": "C4"}, {"value": "-0.0071834527", "module": "D"}]}}, {"referenceToLCIAMethodDataSet": {"shortDescription": [{"value": "Potenzial für den abiotischen Abbau nicht fossiler Ressourcen (ADPE)", "lang": "de"}, {"value": "Abiotic depletion potential for non fossil resources (ADPE)", "lang": "en"}], "type": "LCIA method data set", "refObjectId": "b2ad6494-c78d-11e6-9d9d-cec0c932ce01", "uri": "../lciamethods/b2ad6494-c78d-11e6-9d9d-cec0c932ce01.xml"}, "other": {"anies": [{"name": "referenceToUnitGroupDataSet", "value": {"shortDescription": [{"value": "kg Sb-Äq.", "lang": "de"}], "type": "unit group data set", "refObjectId": "54ccd2d9-a32a-4fc2-923d-f2c8c93e89d4", "uri": "../unitgroups/54ccd2d9-a32a-4fc2-923d-f2c8c93e89d4.xml"}}, {"value": "6.9488168894E-05", "module": "A1-A3"}, {"value": "0", "module": "C1"}, {"value": "1.2380588E-08", "module": "C2"}, {"value": "6.5896516E-09", "module": "C3"}, {"value": "0", "module": "C4"}, {"value": "-6.2725665E-05", "module": "D"}]}}, {"referenceToLCIAMethodDataSet": {"shortDescription": [{"value": "Potenzial für den abiotischen Abbau fossiler Brennstoffe (ADPF)", "lang": "de"}, {"value": "Abiotic depletion potential for fossil resources (ADPF)", "lang": "en"}], "type": "LCIA method data set", "refObjectId": "b2ad6110-c78d-11e6-9d9d-cec0c932ce01", "uri": "../lciamethods/b2ad6110-c78d-11e6-9d9d-cec0c932ce01.xml"}, "other": {"anies": [{"name": "referenceToUnitGroupDataSet", "value": {"shortDescription": [{"value": "MJ", "lang": "de"}], "type": "unit group data set", "refObjectId": "93a60a57-a3c8-11da-a746-0800200c9a66", "uri": "../unitgroups/93a60a57-a3c8-11da-a746-0800200c9a66.xml"}}, {"value": "26.13862051", "module": "A1-A3"}, {"value": "0", "module": "C1"}, {"value": "0.084155371", "module": "C2"}, {"value": "0.055035648", "module": "C3"}, {"value": "0", "module": "C4"}, {"value": "-16.043557", "module": "D"}]}}, {"referenceToLCIAMethodDataSet": {"shortDescription": [{"value": "Wassernutzung (WDP)", "lang": "de"}, {"value": "Water use (WDP)", "lang": "en"}], "type": "LCIA method data set", "refObjectId": "b2ad66ce-c78d-11e6-9d9d-cec0c932ce01", "uri": "../lciamethods/b2ad66ce-c78d-11e6-9d9d-cec0c932ce01.xml"}, "other": {"anies": [{"name": "referenceToUnitGroupDataSet", "value": {"shortDescription": [{"value": "m^(3) Welt-Äq. entzogen", "lang": "de"}], "type": "unit group data set", "refObjectId": "6ae2df01-888e-46c8-b17d-49fa3869b476", "uri": "../unitgroups/6ae2df01-888e-46c8-b17d-49fa3869b476.xml"}}, {"value": "0.9341664239", "module": "A1-A3"}, {"value": "0", "module": "C1"}, {"value": "0.00028954139", "module": "C2"}, {"value": "0.0019321937", "module": "C3"}, {"value": "0", "module": "C4"}, {"value": "-0.40251308", "module": "D"}]}}, {"referenceToLCIAMethodDataSet": {"shortDescription": [{"value": "Auftreten von Krankheiten aufgrund von Feinstaubemissionen (PM)", "lang": "de"}, {"value": "Incidence of disease due to PM emissions (PM)", "lang": "en"}], "type": "LCIA method data set", "refObjectId": "b5c602c6-def3-11e6-bf01-fe55135034f3", "uri": "../lciamethods/b5c602c6-def3-11e6-bf01-fe55135034f3.xml"}, "other": {"anies": [{"name": "referenceToUnitGroupDataSet", "value": {"shortDescription": [{"value": "Krankheitsfälle", "lang": "de"}], "type": "unit group data set", "refObjectId": "3883559b-648f-4afc-8ba2-0bd24f3affa3", "uri": "../unitgroups/3883559b-648f-4afc-8ba2-0bd24f3affa3.xml"}}, {"value": "2.005550042E-07", "module": "A1-A3"}, {"value": "0", "module": "C1"}, {"value": "6.3500799E-10", "module": "C2"}, {"value": "3.9010091E-10", "module": "C3"}, {"value": "0", "module": "C4"}, {"value": "-1.2346887E-07", "module": "D"}]}}, {"referenceToLCIAMethodDataSet": {"shortDescription": [{"value": "Wirkung durch Exposition des Menschen mit U235 (IR)", "lang": "de"}, {"value": "Human exposure efficiency relative to U235 (IR)", "lang": "en"}], "type": "LCIA method data set", "refObjectId": "b5c632be-def3-11e6-bf01-fe55135034f3", "uri": "../lciamethods/b5c632be-def3-11e6-bf01-fe55135034f3.xml"}, "other": {"anies": [{"name": "referenceToUnitGroupDataSet", "value": {"shortDescription": [{"value": "kBq U235-Äq.", "lang": "de"}], "type": "unit group data set", "refObjectId": "456b05bf-1415-44a9-9993-02452f554c09", "uri": "../unitgroups/456b05bf-1415-44a9-9993-02452f554c09.xml"}}, {"value": "0.1357021213", "module": "A1-A3"}, {"value": "0", "module": "C1"}, {"value": "0.00042572909", "module": "C2"}, {"value": "0.00024908171", "module": "C3"}, {"value": "0", "module": "C4"}, {"value": "-0.066035351", "module": "D"}]}}, {"referenceToLCIAMethodDataSet": {"shortDescription": [{"value": "Toxizitätsvergleichseinheit für Ökosysteme (ETP-fw)", "lang": "de"}, {"value": "Comparative toxic unit for ecosystems (ETP-fw)", "lang": "en"}], "type": "LCIA method data set", "refObjectId": "ee1082d1-b0f7-43ca-a1f0-21e2a4a74511", "uri": "../lciamethods/ee1082d1-b0f7-43ca-a1f0-21e2a4a74511.xml"}, "other": {"anies": [{"name": "referenceToUnitGroupDataSet", "value": {"shortDescription": [{"value": "CTUe", "lang": "de"}], "type": "unit group data set", "refObjectId": "aa959ded-f1eb-4efb-9c5c-2d60be36b3e6", "uri": "../unitgroups/aa959ded-f1eb-4efb-9c5c-2d60be36b3e6.xml"}}, {"value": "86.56089244", "module": "A1-A3"}, {"value": "0", "module": "C1"}, {"value": "0.065736562", "module": "C2"}, {"value": "0.039415201", "module": "C3"}, {"value": "0", "module": "C4"}, {"value": "-63.457184", "module": "D"}]}}, {"referenceToLCIAMethodDataSet": {"shortDescription": [{"value": "Toxizitätsvergleichseinheit für Menschen (krebserregend) (HTP-c)", "lang": "de"}, {"value": "Comparative toxic unit for humans (carcinogenic) (HTP-c)", "lang": "en"}], "type": "LCIA method data set", "refObjectId": "2299222a-bbd8-474f-9d4f-4dd1f18aea7c", "uri": "../lciamethods/2299222a-bbd8-474f-9d4f-4dd1f18aea7c.xml"}, "other": {"anies": [{"name": "referenceToUnitGroupDataSet", "value": {"shortDescription": [{"value": "CTUh", "lang": "de"}], "type": "unit group data set", "refObjectId": "d4c9523e-2d7e-49fd-8469-998f547d3a70", "uri": "../unitgroups/d4c9523e-2d7e-49fd-8469-998f547d3a70.xml"}}, {"value": "1.7861642235E-08", "module": "A1-A3"}, {"value": "0", "module": "C1"}, {"value": "1.8183862E-12", "module": "C2"}, {"value": "1.2233901E-12", "module": "C3"}, {"value": "0", "module": "C4"}, {"value": "-9.8154163E-09", "module": "D"}]}}, {"referenceToLCIAMethodDataSet": {"shortDescription": [{"value": "Toxizitätsvergleichseinheit für Menschen (nicht krebserregend) (HTP-nc)", "lang": "de"}, {"value": "Comparative toxic unit for humans (noncarcinogenic) (HTP-nc)", "lang": "en"}], "type": "LCIA method data set", "refObjectId": "3af763a5-b7a1-48c9-9cee-1f223481fcef", "uri": "../lciamethods/3af763a5-b7a1-48c9-9cee-1f223481fcef.xml"}, "other": {"anies": [{"name": "referenceToUnitGroupDataSet", "value": {"shortDescription": [{"value": "CTUh", "lang": "de"}], "type": "unit group data set", "refObjectId": "d4c9523e-2d7e-49fd-8469-998f547d3a70", "uri": "../unitgroups/d4c9523e-2d7e-49fd-8469-998f547d3a70.xml"}}, {"value": "8.657579913E-08", "module": "A1-A3"}, {"value": "0", "module": "C1"}, {"value": "7.1936692E-11", "module": "C2"}, {"value": "3.0019907E-11", "module": "C3"}, {"value": "0", "module": "C4"}, {"value": "-4.8185509E-08", "module": "D"}]}}, {"referenceToLCIAMethodDataSet": {"shortDescription": [{"value": "Bodenqualitätsindex (SQP)", "lang": "de"}, {"value": "Soil quality index (SQP)", "lang": "en"}], "type": "LCIA method data set", "refObjectId": "b2ad6890-c78d-11e6-9d9d-cec0c932ce01", "uri": "../lciamethods/b2ad6890-c78d-11e6-9d9d-cec0c932ce01.xml"}, "other": {"anies": [{"name": "referenceToUnitGroupDataSet", "value": {"shortDescription": [{"value": "SQP", "lang": "de"}], "type": "unit group data set", "refObjectId": "f130951c-e67f-4f7f-8dd4-665de3974e18", "uri": "../unitgroups/f130951c-e67f-4f7f-8dd4-665de3974e18.xml"}}, {"value": "9.89049772", "module": "A1-A3"}, {"value": "0", "module": "C1"}, {"value": "0.096799619", "module": "C2"}, {"value": "0.10135424", "module": "C3"}, {"value": "0", "module": "C4"}, {"value": "-6.0400549", "module": "D"}]}}]}, "otherAttributes": {"{http://www.indata.network/EPD/2019}epd-version": "1.2"}, "version": "1.1", "locations": "../ILCDLocations.xml"}