{"processInformation": {"dataSetInformation": {"UUID": "313a4a06-07ce-41e4-a693-a756ec562589", "name": {"baseName": [{"value": "Huppenberger-Maxit Strohbauplatten Rohdichte 220 kg/m³", "lang": "de"}, {"value": "Huppenberger-Maxit straw panels gross density 220 kg/m³", "lang": "en"}], "functionalUnitFlowProperties": [{"value": "1 m3 Strohplatten Produkt mit 220 kg pro m3", "lang": "de"}]}, "synonyms": [{"value": "Stroh Nachwachsende Rohstoffe Dämmstoff Matte Fasern", "lang": "de"}], "classificationInformation": {"classification": [{"class": [{"value": "Dämmstoffe", "level": 0, "classId": "2"}, {"value": "Stroh", "level": 1, "classId": "2.23"}, {"value": "Strohplatten", "level": 2, "classId": "2.23.02"}], "name": "OEKOBAU.DAT"}]}, "generalComment": [{"value": "Die vorliegende Umwelt-Produktdeklaration deklariert eine Strohplatte, produziert am Standort St. Oswald-Riedlhütte, Deutschland.", "lang": "de"}], "other": {"anies": [{"margins": 0.0, "description": [{"value": "keine", "lang": "de"}]}, {"scenario": [{"description": [{"value": "100% Thermische Verwertung"}], "name": "Energierückgewinnung", "default": true}, {"description": [{"value": "100% Recycling"}], "name": "Recycling", "default": false}]}, "<ns11:modules xmlns:ns11=\"http://openlca.org/epd_ilcd\" xmlns=\"http://lca.jrc.it/ILCD/Process\" xmlns:c=\"http://lca.jrc.it/ILCD/Contact\" xmlns:common=\"http://lca.jrc.it/ILCD/Common\" xmlns:epd=\"http://www.iai.kit.edu/EPD/2013\" xmlns:epd2=\"http://www.indata.network/EPD/2019\" xmlns:f=\"http://lca.jrc.it/ILCD/Flow\" xmlns:fp=\"http://lca.jrc.it/ILCD/FlowProperty\" xmlns:m=\"http://lca.jrc.it/ILCD/LCIAMethod\" xmlns:ns10=\"http://www.okworx.com/ILCD/Extensions/2018/Profile\" xmlns:s=\"http://lca.jrc.it/ILCD/Source\" xmlns:u=\"http://lca.jrc.it/ILCD/UnitGroup\" name=\"A1\"/>", "<ns11:modules xmlns:ns11=\"http://openlca.org/epd_ilcd\" xmlns=\"http://lca.jrc.it/ILCD/Process\" xmlns:c=\"http://lca.jrc.it/ILCD/Contact\" xmlns:common=\"http://lca.jrc.it/ILCD/Common\" xmlns:epd=\"http://www.iai.kit.edu/EPD/2013\" xmlns:epd2=\"http://www.indata.network/EPD/2019\" xmlns:f=\"http://lca.jrc.it/ILCD/Flow\" xmlns:fp=\"http://lca.jrc.it/ILCD/FlowProperty\" xmlns:m=\"http://lca.jrc.it/ILCD/LCIAMethod\" xmlns:ns10=\"http://www.okworx.com/ILCD/Extensions/2018/Profile\" xmlns:s=\"http://lca.jrc.it/ILCD/Source\" xmlns:u=\"http://lca.jrc.it/ILCD/UnitGroup\" name=\"A2\"/>", "<ns11:modules xmlns:ns11=\"http://openlca.org/epd_ilcd\" xmlns=\"http://lca.jrc.it/ILCD/Process\" xmlns:c=\"http://lca.jrc.it/ILCD/Contact\" xmlns:common=\"http://lca.jrc.it/ILCD/Common\" xmlns:epd=\"http://www.iai.kit.edu/EPD/2013\" xmlns:epd2=\"http://www.indata.network/EPD/2019\" xmlns:f=\"http://lca.jrc.it/ILCD/Flow\" xmlns:fp=\"http://lca.jrc.it/ILCD/FlowProperty\" xmlns:m=\"http://lca.jrc.it/ILCD/LCIAMethod\" xmlns:ns10=\"http://www.okworx.com/ILCD/Extensions/2018/Profile\" xmlns:s=\"http://lca.jrc.it/ILCD/Source\" xmlns:u=\"http://lca.jrc.it/ILCD/UnitGroup\" name=\"A3\"/>", "<ns11:modules xmlns:ns11=\"http://openlca.org/epd_ilcd\" xmlns=\"http://lca.jrc.it/ILCD/Process\" xmlns:c=\"http://lca.jrc.it/ILCD/Contact\" xmlns:common=\"http://lca.jrc.it/ILCD/Common\" xmlns:epd=\"http://www.iai.kit.edu/EPD/2013\" xmlns:epd2=\"http://www.indata.network/EPD/2019\" xmlns:f=\"http://lca.jrc.it/ILCD/Flow\" xmlns:fp=\"http://lca.jrc.it/ILCD/FlowProperty\" xmlns:m=\"http://lca.jrc.it/ILCD/LCIAMethod\" xmlns:ns10=\"http://www.okworx.com/ILCD/Extensions/2018/Profile\" xmlns:s=\"http://lca.jrc.it/ILCD/Source\" xmlns:u=\"http://lca.jrc.it/ILCD/UnitGroup\" name=\"A1-A3\"/>", "<ns11:modules xmlns:ns11=\"http://openlca.org/epd_ilcd\" xmlns=\"http://lca.jrc.it/ILCD/Process\" xmlns:c=\"http://lca.jrc.it/ILCD/Contact\" xmlns:common=\"http://lca.jrc.it/ILCD/Common\" xmlns:epd=\"http://www.iai.kit.edu/EPD/2013\" xmlns:epd2=\"http://www.indata.network/EPD/2019\" xmlns:f=\"http://lca.jrc.it/ILCD/Flow\" xmlns:fp=\"http://lca.jrc.it/ILCD/FlowProperty\" xmlns:m=\"http://lca.jrc.it/ILCD/LCIAMethod\" xmlns:ns10=\"http://www.okworx.com/ILCD/Extensions/2018/Profile\" xmlns:s=\"http://lca.jrc.it/ILCD/Source\" xmlns:u=\"http://lca.jrc.it/ILCD/UnitGroup\" name=\"A4\"/>", "<ns11:modules xmlns:ns11=\"http://openlca.org/epd_ilcd\" xmlns=\"http://lca.jrc.it/ILCD/Process\" xmlns:c=\"http://lca.jrc.it/ILCD/Contact\" xmlns:common=\"http://lca.jrc.it/ILCD/Common\" xmlns:epd=\"http://www.iai.kit.edu/EPD/2013\" xmlns:epd2=\"http://www.indata.network/EPD/2019\" xmlns:f=\"http://lca.jrc.it/ILCD/Flow\" xmlns:fp=\"http://lca.jrc.it/ILCD/FlowProperty\" xmlns:m=\"http://lca.jrc.it/ILCD/LCIAMethod\" xmlns:ns10=\"http://www.okworx.com/ILCD/Extensions/2018/Profile\" xmlns:s=\"http://lca.jrc.it/ILCD/Source\" xmlns:u=\"http://lca.jrc.it/ILCD/UnitGroup\" name=\"A5\"/>", "<ns11:modules xmlns:ns11=\"http://openlca.org/epd_ilcd\" xmlns=\"http://lca.jrc.it/ILCD/Process\" xmlns:c=\"http://lca.jrc.it/ILCD/Contact\" xmlns:common=\"http://lca.jrc.it/ILCD/Common\" xmlns:epd=\"http://www.iai.kit.edu/EPD/2013\" xmlns:epd2=\"http://www.indata.network/EPD/2019\" xmlns:f=\"http://lca.jrc.it/ILCD/Flow\" xmlns:fp=\"http://lca.jrc.it/ILCD/FlowProperty\" xmlns:m=\"http://lca.jrc.it/ILCD/LCIAMethod\" xmlns:ns10=\"http://www.okworx.com/ILCD/Extensions/2018/Profile\" xmlns:s=\"http://lca.jrc.it/ILCD/Source\" xmlns:u=\"http://lca.jrc.it/ILCD/UnitGroup\" name=\"B1\"/>", "<ns11:modules xmlns:ns11=\"http://openlca.org/epd_ilcd\" xmlns=\"http://lca.jrc.it/ILCD/Process\" xmlns:c=\"http://lca.jrc.it/ILCD/Contact\" xmlns:common=\"http://lca.jrc.it/ILCD/Common\" xmlns:epd=\"http://www.iai.kit.edu/EPD/2013\" xmlns:epd2=\"http://www.indata.network/EPD/2019\" xmlns:f=\"http://lca.jrc.it/ILCD/Flow\" xmlns:fp=\"http://lca.jrc.it/ILCD/FlowProperty\" xmlns:m=\"http://lca.jrc.it/ILCD/LCIAMethod\" xmlns:ns10=\"http://www.okworx.com/ILCD/Extensions/2018/Profile\" xmlns:s=\"http://lca.jrc.it/ILCD/Source\" xmlns:u=\"http://lca.jrc.it/ILCD/UnitGroup\" name=\"B2\"/>", "<ns11:modules xmlns:ns11=\"http://openlca.org/epd_ilcd\" xmlns=\"http://lca.jrc.it/ILCD/Process\" xmlns:c=\"http://lca.jrc.it/ILCD/Contact\" xmlns:common=\"http://lca.jrc.it/ILCD/Common\" xmlns:epd=\"http://www.iai.kit.edu/EPD/2013\" xmlns:epd2=\"http://www.indata.network/EPD/2019\" xmlns:f=\"http://lca.jrc.it/ILCD/Flow\" xmlns:fp=\"http://lca.jrc.it/ILCD/FlowProperty\" xmlns:m=\"http://lca.jrc.it/ILCD/LCIAMethod\" xmlns:ns10=\"http://www.okworx.com/ILCD/Extensions/2018/Profile\" xmlns:s=\"http://lca.jrc.it/ILCD/Source\" xmlns:u=\"http://lca.jrc.it/ILCD/UnitGroup\" name=\"B3\"/>", "<ns11:modules xmlns:ns11=\"http://openlca.org/epd_ilcd\" xmlns=\"http://lca.jrc.it/ILCD/Process\" xmlns:c=\"http://lca.jrc.it/ILCD/Contact\" xmlns:common=\"http://lca.jrc.it/ILCD/Common\" xmlns:epd=\"http://www.iai.kit.edu/EPD/2013\" xmlns:epd2=\"http://www.indata.network/EPD/2019\" xmlns:f=\"http://lca.jrc.it/ILCD/Flow\" xmlns:fp=\"http://lca.jrc.it/ILCD/FlowProperty\" xmlns:m=\"http://lca.jrc.it/ILCD/LCIAMethod\" xmlns:ns10=\"http://www.okworx.com/ILCD/Extensions/2018/Profile\" xmlns:s=\"http://lca.jrc.it/ILCD/Source\" xmlns:u=\"http://lca.jrc.it/ILCD/UnitGroup\" name=\"B4\"/>", "<ns11:modules xmlns:ns11=\"http://openlca.org/epd_ilcd\" xmlns=\"http://lca.jrc.it/ILCD/Process\" xmlns:c=\"http://lca.jrc.it/ILCD/Contact\" xmlns:common=\"http://lca.jrc.it/ILCD/Common\" xmlns:epd=\"http://www.iai.kit.edu/EPD/2013\" xmlns:epd2=\"http://www.indata.network/EPD/2019\" xmlns:f=\"http://lca.jrc.it/ILCD/Flow\" xmlns:fp=\"http://lca.jrc.it/ILCD/FlowProperty\" xmlns:m=\"http://lca.jrc.it/ILCD/LCIAMethod\" xmlns:ns10=\"http://www.okworx.com/ILCD/Extensions/2018/Profile\" xmlns:s=\"http://lca.jrc.it/ILCD/Source\" xmlns:u=\"http://lca.jrc.it/ILCD/UnitGroup\" name=\"B5\"/>", "<ns11:modules xmlns:ns11=\"http://openlca.org/epd_ilcd\" xmlns=\"http://lca.jrc.it/ILCD/Process\" xmlns:c=\"http://lca.jrc.it/ILCD/Contact\" xmlns:common=\"http://lca.jrc.it/ILCD/Common\" xmlns:epd=\"http://www.iai.kit.edu/EPD/2013\" xmlns:epd2=\"http://www.indata.network/EPD/2019\" xmlns:f=\"http://lca.jrc.it/ILCD/Flow\" xmlns:fp=\"http://lca.jrc.it/ILCD/FlowProperty\" xmlns:m=\"http://lca.jrc.it/ILCD/LCIAMethod\" xmlns:ns10=\"http://www.okworx.com/ILCD/Extensions/2018/Profile\" xmlns:s=\"http://lca.jrc.it/ILCD/Source\" xmlns:u=\"http://lca.jrc.it/ILCD/UnitGroup\" name=\"B6\"/>", "<ns11:modules xmlns:ns11=\"http://openlca.org/epd_ilcd\" xmlns=\"http://lca.jrc.it/ILCD/Process\" xmlns:c=\"http://lca.jrc.it/ILCD/Contact\" xmlns:common=\"http://lca.jrc.it/ILCD/Common\" xmlns:epd=\"http://www.iai.kit.edu/EPD/2013\" xmlns:epd2=\"http://www.indata.network/EPD/2019\" xmlns:f=\"http://lca.jrc.it/ILCD/Flow\" xmlns:fp=\"http://lca.jrc.it/ILCD/FlowProperty\" xmlns:m=\"http://lca.jrc.it/ILCD/LCIAMethod\" xmlns:ns10=\"http://www.okworx.com/ILCD/Extensions/2018/Profile\" xmlns:s=\"http://lca.jrc.it/ILCD/Source\" xmlns:u=\"http://lca.jrc.it/ILCD/UnitGroup\" name=\"B7\"/>", "<ns11:modules xmlns:ns11=\"http://openlca.org/epd_ilcd\" xmlns=\"http://lca.jrc.it/ILCD/Process\" xmlns:c=\"http://lca.jrc.it/ILCD/Contact\" xmlns:common=\"http://lca.jrc.it/ILCD/Common\" xmlns:epd=\"http://www.iai.kit.edu/EPD/2013\" xmlns:epd2=\"http://www.indata.network/EPD/2019\" xmlns:f=\"http://lca.jrc.it/ILCD/Flow\" xmlns:fp=\"http://lca.jrc.it/ILCD/FlowProperty\" xmlns:m=\"http://lca.jrc.it/ILCD/LCIAMethod\" xmlns:ns10=\"http://www.okworx.com/ILCD/Extensions/2018/Profile\" xmlns:s=\"http://lca.jrc.it/ILCD/Source\" xmlns:u=\"http://lca.jrc.it/ILCD/UnitGroup\" name=\"C1\" scenario=\"Energierückgewinnung\"/>", "<ns11:modules xmlns:ns11=\"http://openlca.org/epd_ilcd\" xmlns=\"http://lca.jrc.it/ILCD/Process\" xmlns:c=\"http://lca.jrc.it/ILCD/Contact\" xmlns:common=\"http://lca.jrc.it/ILCD/Common\" xmlns:epd=\"http://www.iai.kit.edu/EPD/2013\" xmlns:epd2=\"http://www.indata.network/EPD/2019\" xmlns:f=\"http://lca.jrc.it/ILCD/Flow\" xmlns:fp=\"http://lca.jrc.it/ILCD/FlowProperty\" xmlns:m=\"http://lca.jrc.it/ILCD/LCIAMethod\" xmlns:ns10=\"http://www.okworx.com/ILCD/Extensions/2018/Profile\" xmlns:s=\"http://lca.jrc.it/ILCD/Source\" xmlns:u=\"http://lca.jrc.it/ILCD/UnitGroup\" name=\"C2\" scenario=\"Energierückgewinnung\"/>", "<ns11:modules xmlns:ns11=\"http://openlca.org/epd_ilcd\" xmlns=\"http://lca.jrc.it/ILCD/Process\" xmlns:c=\"http://lca.jrc.it/ILCD/Contact\" xmlns:common=\"http://lca.jrc.it/ILCD/Common\" xmlns:epd=\"http://www.iai.kit.edu/EPD/2013\" xmlns:epd2=\"http://www.indata.network/EPD/2019\" xmlns:f=\"http://lca.jrc.it/ILCD/Flow\" xmlns:fp=\"http://lca.jrc.it/ILCD/FlowProperty\" xmlns:m=\"http://lca.jrc.it/ILCD/LCIAMethod\" xmlns:ns10=\"http://www.okworx.com/ILCD/Extensions/2018/Profile\" xmlns:s=\"http://lca.jrc.it/ILCD/Source\" xmlns:u=\"http://lca.jrc.it/ILCD/UnitGroup\" name=\"C3\" scenario=\"Energierückgewinnung\"/>", "<ns11:modules xmlns:ns11=\"http://openlca.org/epd_ilcd\" xmlns=\"http://lca.jrc.it/ILCD/Process\" xmlns:c=\"http://lca.jrc.it/ILCD/Contact\" xmlns:common=\"http://lca.jrc.it/ILCD/Common\" xmlns:epd=\"http://www.iai.kit.edu/EPD/2013\" xmlns:epd2=\"http://www.indata.network/EPD/2019\" xmlns:f=\"http://lca.jrc.it/ILCD/Flow\" xmlns:fp=\"http://lca.jrc.it/ILCD/FlowProperty\" xmlns:m=\"http://lca.jrc.it/ILCD/LCIAMethod\" xmlns:ns10=\"http://www.okworx.com/ILCD/Extensions/2018/Profile\" xmlns:s=\"http://lca.jrc.it/ILCD/Source\" xmlns:u=\"http://lca.jrc.it/ILCD/UnitGroup\" name=\"C4\" scenario=\"Energierückgewinnung\"/>", "<ns11:modules xmlns:ns11=\"http://openlca.org/epd_ilcd\" xmlns=\"http://lca.jrc.it/ILCD/Process\" xmlns:c=\"http://lca.jrc.it/ILCD/Contact\" xmlns:common=\"http://lca.jrc.it/ILCD/Common\" xmlns:epd=\"http://www.iai.kit.edu/EPD/2013\" xmlns:epd2=\"http://www.indata.network/EPD/2019\" xmlns:f=\"http://lca.jrc.it/ILCD/Flow\" xmlns:fp=\"http://lca.jrc.it/ILCD/FlowProperty\" xmlns:m=\"http://lca.jrc.it/ILCD/LCIAMethod\" xmlns:ns10=\"http://www.okworx.com/ILCD/Extensions/2018/Profile\" xmlns:s=\"http://lca.jrc.it/ILCD/Source\" xmlns:u=\"http://lca.jrc.it/ILCD/UnitGroup\" name=\"D\" scenario=\"Energierückgewinnung\"/>", "<ns11:modules xmlns:ns11=\"http://openlca.org/epd_ilcd\" xmlns=\"http://lca.jrc.it/ILCD/Process\" xmlns:c=\"http://lca.jrc.it/ILCD/Contact\" xmlns:common=\"http://lca.jrc.it/ILCD/Common\" xmlns:epd=\"http://www.iai.kit.edu/EPD/2013\" xmlns:epd2=\"http://www.indata.network/EPD/2019\" xmlns:f=\"http://lca.jrc.it/ILCD/Flow\" xmlns:fp=\"http://lca.jrc.it/ILCD/FlowProperty\" xmlns:m=\"http://lca.jrc.it/ILCD/LCIAMethod\" xmlns:ns10=\"http://www.okworx.com/ILCD/Extensions/2018/Profile\" xmlns:s=\"http://lca.jrc.it/ILCD/Source\" xmlns:u=\"http://lca.jrc.it/ILCD/UnitGroup\" name=\"C1\" scenario=\"Recycling\"/>", "<ns11:modules xmlns:ns11=\"http://openlca.org/epd_ilcd\" xmlns=\"http://lca.jrc.it/ILCD/Process\" xmlns:c=\"http://lca.jrc.it/ILCD/Contact\" xmlns:common=\"http://lca.jrc.it/ILCD/Common\" xmlns:epd=\"http://www.iai.kit.edu/EPD/2013\" xmlns:epd2=\"http://www.indata.network/EPD/2019\" xmlns:f=\"http://lca.jrc.it/ILCD/Flow\" xmlns:fp=\"http://lca.jrc.it/ILCD/FlowProperty\" xmlns:m=\"http://lca.jrc.it/ILCD/LCIAMethod\" xmlns:ns10=\"http://www.okworx.com/ILCD/Extensions/2018/Profile\" xmlns:s=\"http://lca.jrc.it/ILCD/Source\" xmlns:u=\"http://lca.jrc.it/ILCD/UnitGroup\" name=\"C2\" scenario=\"Recycling\"/>", "<ns11:modules xmlns:ns11=\"http://openlca.org/epd_ilcd\" xmlns=\"http://lca.jrc.it/ILCD/Process\" xmlns:c=\"http://lca.jrc.it/ILCD/Contact\" xmlns:common=\"http://lca.jrc.it/ILCD/Common\" xmlns:epd=\"http://www.iai.kit.edu/EPD/2013\" xmlns:epd2=\"http://www.indata.network/EPD/2019\" xmlns:f=\"http://lca.jrc.it/ILCD/Flow\" xmlns:fp=\"http://lca.jrc.it/ILCD/FlowProperty\" xmlns:m=\"http://lca.jrc.it/ILCD/LCIAMethod\" xmlns:ns10=\"http://www.okworx.com/ILCD/Extensions/2018/Profile\" xmlns:s=\"http://lca.jrc.it/ILCD/Source\" xmlns:u=\"http://lca.jrc.it/ILCD/UnitGroup\" name=\"C3\" scenario=\"Recycling\"/>", "<ns11:modules xmlns:ns11=\"http://openlca.org/epd_ilcd\" xmlns=\"http://lca.jrc.it/ILCD/Process\" xmlns:c=\"http://lca.jrc.it/ILCD/Contact\" xmlns:common=\"http://lca.jrc.it/ILCD/Common\" xmlns:epd=\"http://www.iai.kit.edu/EPD/2013\" xmlns:epd2=\"http://www.indata.network/EPD/2019\" xmlns:f=\"http://lca.jrc.it/ILCD/Flow\" xmlns:fp=\"http://lca.jrc.it/ILCD/FlowProperty\" xmlns:m=\"http://lca.jrc.it/ILCD/LCIAMethod\" xmlns:ns10=\"http://www.okworx.com/ILCD/Extensions/2018/Profile\" xmlns:s=\"http://lca.jrc.it/ILCD/Source\" xmlns:u=\"http://lca.jrc.it/ILCD/UnitGroup\" name=\"C4\" scenario=\"Recycling\"/>", "<ns11:modules xmlns:ns11=\"http://openlca.org/epd_ilcd\" xmlns=\"http://lca.jrc.it/ILCD/Process\" xmlns:c=\"http://lca.jrc.it/ILCD/Contact\" xmlns:common=\"http://lca.jrc.it/ILCD/Common\" xmlns:epd=\"http://www.iai.kit.edu/EPD/2013\" xmlns:epd2=\"http://www.indata.network/EPD/2019\" xmlns:f=\"http://lca.jrc.it/ILCD/Flow\" xmlns:fp=\"http://lca.jrc.it/ILCD/FlowProperty\" xmlns:m=\"http://lca.jrc.it/ILCD/LCIAMethod\" xmlns:ns10=\"http://www.okworx.com/ILCD/Extensions/2018/Profile\" xmlns:s=\"http://lca.jrc.it/ILCD/Source\" xmlns:u=\"http://lca.jrc.it/ILCD/UnitGroup\" name=\"D\" scenario=\"Recycling\"/>"]}}, "quantitativeReference": {"referenceToReferenceFlow": [1], "type": "Reference flow(s)"}, "time": {"referenceYear": 2023, "dataSetValidUntil": 2028, "timeRepresentativenessDescription": [{"value": "Die vom Hersteller zur Verfügung gestellten Daten beziehen sich auf das Jahr 2022.", "lang": "de"}], "other": {"anies": [{"name": "publicationDateOfEPD", "value": 1686873600000}]}}, "geography": {"locationOfOperationSupplyOrProduction": {"descriptionOfRestrictions": [{"value": "Die Auslieferung des Produkts erfolgt ausschließlich mittels LKW. Die Transportdistanz ist vom tatsächlichen Einsatzort abhängig, wobei aktuell Deutschland und Österreich relevante Absatzmärkte darstellen. In Abhängigkeit der Vertriebsanteile in diese Länder sowie den entsprechenden durchschnittlichen Transportdistanzen wurde ein repräsentativer Transport abgebildet.", "lang": "de"}, {"value": "The product is delivered exclusively by lorry. The transport distance depends on the actual place of use, with Germany and Austria currently representing relevant sales markets. A representative transport was mapped depending on the share of sales to these countries and the corresponding average transport distances.", "lang": "en"}], "location": "RER"}}, "technology": {"technologyDescriptionAndIncludedProcesses": [{"value": "Betrachtet wird eine am Standort St. Oswald-Riedlhütte (Deutschland) produzierte Strohplatte, die neben dem nachwachsenden Grundstoff Stroh auch Bindemittel (diverse Makromoleküle aus Aminosäure-Gruppen und Fettsäureester) sowie Schimmelhemmer (Afrotin) enthält. Die Platte kann je nach Anwendungsbereich (siehe 2.2) in unterschiedlichen Dichten hergestellt werden, die relative Zusammensetzung variiert dabei nicht. Die in dieser EPD dargestellten Ergebnisse beziehen sich ausschließlich auf die Putzträgerplatte mit einer Dichte von 220 kg/m³. Eine Umrechnung auf Platten mit anderen Dichten ist über das Dichteverhältnis möglich.", "lang": "de"}, {"value": "The strawboard can be used indoors (with the exception of damp rooms) as a non-load-bearing interior finishing board for subsequent plaster coating, for interior room partitioning as a facing layer, as panelling for OSB boards or as ceiling cladding. In addition, it can also be used as an insulating board for interior and exterior solid masonry, as a timber frame and board material in timber construction and as an impact sound board for interior applications.", "lang": "en"}], "technologicalApplicability": [{"value": "Die Strohplatte kann im Innenbereich (mit Ausnahme von Feuchträumen) als nichtragende Innenausbauplatte zur nachträglichen Putzbeschichtung, für die innere Raumbegrenzung als Vorsatzschale, als Beplankung von OSB-Platten oder als Deckenbekleidung eingesetzt werden. Darüber hinaus ist auch die Verwendung als Dämmplatte im Innen- und Außenbereich für Massivmauerwerk, als Holzständerwerk und Plattenwerkstoff im Holzbau sowie als Trittschallplatte im Innenbereich möglich.", "lang": "de"}, {"value": "The insulation mat is used for the following applications (based on the designations from Annex A of ÖNORM EN 16783): \nCavity insulation of exterior and interior walls in timber frame construction and comparable constructions (WH, WTR); interior insulation of exterior walls between a supporting structure (WI); insulation between rafters and timber beams as well as in cavities of corresponding construction, cavity insulation between bearing timbers in the floor and comparable substructures (DZ); interior insulation of ceiling or roof, e.g. insulation under the supporting structure (e.g. rafters), suspended ceiling (DI).\n\nTranslated with www.DeepL.com/Translator (free version)", "lang": "en"}]}}, "modellingAndValidation": {"LCIMethodAndAllocation": {"typeOfDataSet": "EPD", "referenceToLCAMethodDetails": [{"shortDescription": [{"value": "PKR Bau EPD GmbH PKR-Code: 2.22.5 Version 9.0 Stand 25.02.2022 \"Dämmstoffe aus nachwachsenden Rohstoffen\"", "lang": "de"}], "type": "source data set", "refObjectId": "0a226f34-7447-4c89-ad83-f8d21456b86c", "version": "00.00.001"}], "other": {"anies": [{"name": "subType", "value": "specific dataset"}]}}, "dataSourcesTreatmentAndRepresentativeness": {"referenceToDataSource": [{"shortDescription": [{"value": "GaBi database (general)", "lang": "en"}], "type": "source data set", "refObjectId": "28d74cc0-db8b-4d7e-bc44-5f6d56ce0c4a", "version": "00.03.002"}, {"shortDescription": [{"value": "Software: Umberto LCA+", "lang": "de"}], "type": "source data set", "refObjectId": "3b215025-51cc-4bc7-9dfc-d6130a38572b", "version": "00.00.001"}, {"shortDescription": [{"value": "GaBi Database Edition 2021, CUP 2021.02", "lang": "en"}], "type": "source data set", "refObjectId": "90321ffe-9ebb-4946-886c-338efe6fbf26", "version": "00.01.000"}], "useAdviceForDataSet": [{"value": "Anmerkung zur Vergleichbarkeit: Ein Vergleich mit anderen Produkten ist nur mit einer vergleichbaren Anwendung im Gebäude sinnvoll. Grundsätzlich ist eine Gegenüberstellung oder die Bewertung von EPD Daten nur möglich, wenn alle zu vergleichenden Datensätze nach EN 15804 erstellt wurden und die produktspezifischen Leistungsmerkmale berücksichtigt werden.", "lang": "de"}], "other": {"anies": [{"name": "referenceToOriginalEPD", "value": {"shortDescription": {"value": "Bau EPD GmbH EPD GABI MAXIT HUPPENBERGER 2023-1", "defaultValue": "Bau EPD GmbH EPD GABI MAXIT HUPPENBERGER 2023-1", "lstrings": [{"lang": "de", "value": "Bau EPD GmbH EPD GABI MAXIT HUPPENBERGER 2023-1"}, {"lang": "en", "value": "Bau EPD GmbH / EPD-FASBA-2014-1-GABI"}]}, "version": {"version": 5, "majorVersion": 0, "minorVersion": 0, "subMinorVersion": 5, "zero": false, "versionString": "00.00.005"}, "uri": "http://openlca.org/ilcd/resource/sources/ed07cc37-ac91-43e7-9629-c0e795e338c5", "href": "http://openlca.org/ilcd/resource/sources/ed07cc37-ac91-43e7-9629-c0e795e338c5", "type": "source data set", "uuid": {"uuid": "a2ff2202-739c-4fb7-9896-99a7a83b2408"}, "refObjectId": "a2ff2202-739c-4fb7-9896-99a7a83b2408", "versionAsString": "00.00.005", "resourceURLs": ["https://oekobaudat.de/OEKOBAU.DAT/resource/sources/a2ff2202-739c-4fb7-9896-99a7a83b2408/BAU-EPD-MAXHUPP-2023-1-GaBi-Strohplatten-20230616.pdf?version=00.00.005"]}}]}}, "validation": {"review": [{"referenceToNameOfReviewerAndInstitution": [{"shortDescription": [{"value": "Bau EPD GmbH", "lang": "de"}, {"value": "Bau EPD GmbH", "lang": "en"}], "type": "contact data set", "refObjectId": "42398bec-0af8-444e-9221-d40be4c4f553", "version": "00.00.007", "uri": "http://openlca.org/ilcd/resource/contacts/42398bec-0af8-444e-9221-d40be4c4f553"}], "type": "Independent external review"}]}, "complianceDeclarations": {"compliance": [{"referenceToComplianceSystem": {"shortDescription": [{"value": "EN 15804+A2 (EF 3.0)", "lang": "de"}, {"value": "EN 15804+A2 (EF 3.0)", "lang": "en"}], "type": "source data set", "refObjectId": "c0016b33-8cf7-415c-ac6e-deba0d21440d", "version": "00.02.000"}}, {"referenceToComplianceSystem": {"shortDescription": [{"value": "ISO 14025", "lang": "en"}], "type": "source data set", "refObjectId": "4f2eb655-6e44-4874-a95a-e28f5442cd4d", "version": "00.00.001"}}]}}, "administrativeInformation": {"commissionerAndGoal": {"referenceToCommissioner": [{"shortDescription": [{"value": "ARGE Maxit-Huppenberger", "lang": "de"}, {"value": "FASBA e.V.", "lang": "en"}], "type": "contact data set", "refObjectId": "be303203-7e9d-47f4-9291-eb6ffd10aa33", "version": "00.00.003", "uri": "http://openlca.org/ilcd/resource/contacts/9828b42f-275d-4651-9853-7abe6183f6b6"}]}, "dataGenerator": {"referenceToPersonOrEntityGeneratingTheDataSet": [{"shortDescription": [{"value": "IBO Institut für Baubiologie und Bauökologie", "lang": "de"}], "type": "contact data set", "refObjectId": "50fccae1-aef9-4e76-acf5-fe0428976e43", "version": "00.00.003"}]}, "dataEntryBy": {"timeStamp": 1747382315601, "referenceToDataSetFormat": [{"shortDescription": [{"value": "EPD Data Format Extensions v1.2", "lang": "en"}, {"value": "EPD-Datenformaterweiterungen v1.2", "lang": "de"}], "type": "source data set", "refObjectId": "a29449fd-aa2f-4de8-b5d7-4b06b43c6fde", "version": "00.01.000"}, {"shortDescription": [{"value": "ILCD format", "lang": "en"}], "type": "source data set", "refObjectId": "a97a0155-0234-4b87-b4ce-a45da52f2a40", "version": "01.00.000", "uri": "http://lca.jrc.ec.europa.eu/lcainfohub/sample_data/ilcd/sources/ILCD_Format_a97a0155-0234-4b87-b4ce-a45da52f2a40_01.00.000.xml"}], "referenceToPersonOrEntityEnteringTheData": {"shortDescription": [{"value": "Bau EPD GmbH", "lang": "de"}, {"value": "Bau EPD GmbH", "lang": "en"}], "type": "contact data set", "refObjectId": "42398bec-0af8-444e-9221-d40be4c4f553", "version": "00.00.007", "uri": "http://openlca.org/ilcd/resource/contacts/42398bec-0af8-444e-9221-d40be4c4f553"}}, "publicationAndOwnership": {"dataSetVersion": "00.00.055", "referenceToRegistrationAuthority": {"shortDescription": [{"value": "Bau EPD GmbH", "lang": "de"}, {"value": "Bau EPD GmbH", "lang": "en"}], "type": "contact data set", "refObjectId": "42398bec-0af8-444e-9221-d40be4c4f553", "version": "00.00.007", "uri": "http://openlca.org/ilcd/resource/contacts/42398bec-0af8-444e-9221-d40be4c4f553"}, "registrationNumber": "BAU-EPD-MAXHUPP-2023-1-GaBi-Strohplatten", "referenceToOwnershipOfDataSet": {"shortDescription": [{"value": "HempFlax Building Solutions GmbH", "lang": "de"}], "type": "contact data set", "refObjectId": "55fe2616-b9c9-485a-9225-2e1c4cac26a3", "version": "00.00.001"}, "copyright": true, "licenseType": "Free of charge for all users and uses", "accessRestrictions": [{"value": "Keine", "lang": "de"}], "other": {"anies": [{"name": "referenceToPublisher", "value": {"shortDescription": [{"value": "Bau EPD GmbH", "lang": "de"}, {"value": "Bau EPD GmbH", "lang": "en"}], "type": "contact data set", "refObjectId": "42398bec-0af8-444e-9221-d40be4c4f553", "version": "00.00.007", "uri": "http://openlca.org/ilcd/resource/contacts/42398bec-0af8-444e-9221-d40be4c4f553"}}]}}}, "exchanges": {"exchange": [{"dataSetInternalID": 1, "referenceToFlowDataSet": {"shortDescription": [{"value": "Strohplatte Huppenberger Maxit", "lang": "de"}], "type": "flow data set", "refObjectId": "2e959214-0cdf-48dc-8e20-ce01761d47b3", "version": "00.00.011"}, "meanAmount": 1.0, "resultingAmount": 1.0, "referenceFlow": true, "resultingflowAmount": 1.0, "flowProperties": [{"name": [{"lang": "en", "value": "Carbon content (biogenic) - packaging"}], "uuid": "262a541b-209e-44cc-a426-33bce30de7b1", "meanValue": 0.93}, {"name": [{"lang": "en", "value": "Carbon content (biogenic)"}], "uuid": "62e503ce-544a-4599-b2ad-bcea15a7bf20", "meanValue": 74.02}, {"name": [{"lang": "en", "value": "Volume"}, {"lang": "de", "value": "Volumen"}], "uuid": "93a60a56-a3c8-22da-a746-0800200c9a66", "referenceFlowProperty": true, "meanValue": 1.0, "referenceUnit": "m3", "unitGroupUUID": "cd950537-0a98-4044-9ba7-9f9a68d0a504"}], "materialProperties": [{"name": "gross density", "value": "220.0", "unit": "kg/m^3", "unitDescription": "kilograms per cubic metre"}], "typeOfFlow": "Product flow", "classification": {"classHierarchy": "Dämmstoffe / Stroh / Strohplatten", "name": "OEKOBAU.DAT"}}, {"dataSetInternalID": 2, "referenceToFlowDataSet": {"shortDescription": [{"value": "Use of renewable primary energy (PERE)", "lang": "en"}, {"value": "Erneuerbare Primärenergie als Energieträger (PERE)", "lang": "de"}, {"value": "Uso de energía primaria renovable excluyendo los recursos de energía primaria renovable utilizada como materia prima (PERE)", "lang": "es"}], "type": "flow data set", "refObjectId": "20f32be5-0398-4288-9b6d-accddd195317", "version": "38.00.000", "uri": "../flows/20f32be5-0398-4288-9b6d-accddd195317.xml"}, "exchange direction": "INPUT", "meanAmount": 0.0, "other": {"anies": [{"value": "361.7340072464695", "module": "A1-A3"}, {"value": "12.589381154778645", "module": "A4"}, {"value": "77.68447546291216", "module": "A5"}, {"value": "0.0", "module": "B1"}, {"value": "0.0", "module": "B2"}, {"value": "0.0", "module": "B3"}, {"value": "0.0", "module": "B4"}, {"value": "0.0", "module": "B5"}, {"value": "0.0", "module": "B6"}, {"value": "0.0", "module": "B7"}, {"value": "0.0", "module": "C1", "scenario": "Energierückgewinnung"}, {"value": "3.8736557399318774", "module": "C2", "scenario": "Energierückgewinnung"}, {"value": "2984.492250234223", "module": "C3", "scenario": "Energierückgewinnung"}, {"value": "0.0", "module": "C4", "scenario": "Energierückgewinnung"}, {"value": "-424.9019915339592", "module": "D", "scenario": "Energierückgewinnung"}, {"value": "0.0", "module": "C1", "scenario": "Recycling"}, {"value": "3.8736557399318774", "module": "C2", "scenario": "Recycling"}, {"value": "2939.5078811741123", "module": "C3", "scenario": "Recycling"}, {"value": "0.0", "module": "C4", "scenario": "Recycling"}, {"value": "-7.839800363598327", "module": "D", "scenario": "Recycling"}, {"name": "referenceToUnitGroupDataSet", "value": {"shortDescription": [{"value": "MJ", "lang": "en"}], "type": "unit group data set", "refObjectId": "93a60a57-a3c8-11da-a746-0800200c9a66", "version": "03.00.000", "uri": "../unitgroups/93a60a57-a3c8-11da-a746-0800200c9a66.xml"}}]}, "flowProperties": [], "typeOfFlow": "Other flow", "classification": {"classHierarchy": "Quantities", "name": "GaBiCategories"}}, {"dataSetInternalID": 3, "referenceToFlowDataSet": {"shortDescription": [{"value": "Use of renewable primary energy resources used as raw materials (PERM)", "lang": "en"}, {"value": "Erneuerbare Primärenergie zur stofflichen Nutzung (PERM)", "lang": "de"}, {"value": "Uso de energía primaria renovable utilizada como materia prima (PERM)", "lang": "es"}], "type": "flow data set", "refObjectId": "fb3ec0de-548d-4508-aea5-00b73bf6f702", "version": "38.00.000", "uri": "../flows/fb3ec0de-548d-4508-aea5-00b73bf6f702.xml"}, "exchange direction": "INPUT", "meanAmount": 0.0, "other": {"anies": [{"value": "3001.0107707796997", "module": "A1-A3"}, {"value": "0.0", "module": "A4"}, {"value": "-33.303932318161614", "module": "A5"}, {"value": "0.0", "module": "B1"}, {"value": "0.0", "module": "B2"}, {"value": "0.0", "module": "B3"}, {"value": "0.0", "module": "B4"}, {"value": "0.0", "module": "B5"}, {"value": "0.0", "module": "B6"}, {"value": "0.0", "module": "B7"}, {"value": "0.0", "module": "C1", "scenario": "Energierückgewinnung"}, {"value": "0.0", "module": "C2", "scenario": "Energierückgewinnung"}, {"value": "-2967.706838461538", "module": "C3", "scenario": "Energierückgewinnung"}, {"value": "0.0", "module": "C4", "scenario": "Energierückgewinnung"}, {"value": "0.0", "module": "D", "scenario": "Energierückgewinnung"}, {"value": "0.0", "module": "C1", "scenario": "Recycling"}, {"value": "0.0", "module": "C2", "scenario": "Recycling"}, {"value": "-2967.706838461538", "module": "C3", "scenario": "Recycling"}, {"value": "0.0", "module": "C4", "scenario": "Recycling"}, {"value": "0.0", "module": "D", "scenario": "Recycling"}, {"name": "referenceToUnitGroupDataSet", "value": {"shortDescription": [{"value": "MJ", "lang": "en"}], "type": "unit group data set", "refObjectId": "93a60a57-a3c8-11da-a746-0800200c9a66", "version": "03.00.000", "uri": "../unitgroups/93a60a57-a3c8-11da-a746-0800200c9a66.xml"}}]}, "flowProperties": [], "typeOfFlow": "Other flow", "classification": {"classHierarchy": "Quantities", "name": "GaBiCategories"}}, {"dataSetInternalID": 4, "referenceToFlowDataSet": {"shortDescription": [{"value": "Total use of renewable primary energy resources (PERT)", "lang": "en"}, {"value": "Total erneuerbare Primärenergie (PERT)", "lang": "de"}, {"value": "Uso total de la energía primaria renovable (energía primaria y recursos de energía primaria renovable utilizada como materia prima) (PERT)", "lang": "es"}], "type": "flow data set", "refObjectId": "53f97275-fa8a-4cdd-9024-65936002acd0", "version": "30.00.000", "uri": "../flows/53f97275-fa8a-4cdd-9024-65936002acd0.xml"}, "exchange direction": "INPUT", "meanAmount": 0.0, "other": {"anies": [{"value": "3362.744778026169", "module": "A1-A3"}, {"value": "12.589381154778645", "module": "A4"}, {"value": "44.38054314475055", "module": "A5"}, {"value": "0.0", "module": "B1"}, {"value": "0.0", "module": "B2"}, {"value": "0.0", "module": "B3"}, {"value": "0.0", "module": "B4"}, {"value": "0.0", "module": "B5"}, {"value": "0.0", "module": "B6"}, {"value": "0.0", "module": "B7"}, {"value": "0.0", "module": "C1", "scenario": "Energierückgewinnung"}, {"value": "3.8736557399318774", "module": "C2", "scenario": "Energierückgewinnung"}, {"value": "16.78541177268471", "module": "C3", "scenario": "Energierückgewinnung"}, {"value": "0.0", "module": "C4", "scenario": "Energierückgewinnung"}, {"value": "-424.9019915339592", "module": "D", "scenario": "Energierückgewinnung"}, {"value": "0.0", "module": "C1", "scenario": "Recycling"}, {"value": "3.8736557399318774", "module": "C2", "scenario": "Recycling"}, {"value": "-28.198957287425856", "module": "C3", "scenario": "Recycling"}, {"value": "0.0", "module": "C4", "scenario": "Recycling"}, {"value": "-7.839800363598327", "module": "D", "scenario": "Recycling"}, {"name": "referenceToUnitGroupDataSet", "value": {"shortDescription": [{"value": "MJ", "lang": "en"}], "type": "unit group data set", "refObjectId": "93a60a57-a3c8-11da-a746-0800200c9a66", "version": "03.00.000", "uri": "../unitgroups/93a60a57-a3c8-11da-a746-0800200c9a66.xml"}}]}, "flowProperties": [], "typeOfFlow": "Other flow", "classification": {"classHierarchy": "Größen / Umweltliche Größen / EPD EN 15804 / LCI Indikatoren", "name": "GaBiCategories"}}, {"dataSetInternalID": 5, "referenceToFlowDataSet": {"shortDescription": [{"value": "Use of non renewable primary energy (PENRE)", "lang": "en"}, {"value": "Nicht-erneuerbare Primärenergie als Energieträger (PENRE)", "lang": "de"}, {"value": "Uso de energía primaria no renovable, excluyendo los recursos de energía primaria no renovable utilizada como materia prima (PENRE)", "lang": "es"}], "type": "flow data set", "refObjectId": "ac857178-2b45-46ec-892a-a9a4332f0372", "version": "38.00.000", "uri": "../flows/ac857178-2b45-46ec-892a-a9a4332f0372.xml"}, "exchange direction": "INPUT", "meanAmount": 0.0, "other": {"anies": [{"value": "2482.9862530136147", "module": "A1-A3"}, {"value": "210.78798473269012", "module": "A4"}, {"value": "44.65932580458516", "module": "A5"}, {"value": "0.0", "module": "B1"}, {"value": "0.0", "module": "B2"}, {"value": "0.0", "module": "B3"}, {"value": "0.0", "module": "B4"}, {"value": "0.0", "module": "B5"}, {"value": "0.0", "module": "B6"}, {"value": "0.0", "module": "B7"}, {"value": "0.0", "module": "C1", "scenario": "Energierückgewinnung"}, {"value": "64.85784145621224", "module": "C2", "scenario": "Energierückgewinnung"}, {"value": "308.36047208873254", "module": "C3", "scenario": "Energierückgewinnung"}, {"value": "0.0", "module": "C4", "scenario": "Energierückgewinnung"}, {"value": "-1910.6864396612325", "module": "D", "scenario": "Energierückgewinnung"}, {"value": "0.0", "module": "C1", "scenario": "Recycling"}, {"value": "64.85784145621224", "module": "C2", "scenario": "Recycling"}, {"value": "218.855987712496", "module": "C3", "scenario": "Recycling"}, {"value": "0.0", "module": "C4", "scenario": "Recycling"}, {"value": "-95.19281208508585", "module": "D", "scenario": "Recycling"}, {"name": "referenceToUnitGroupDataSet", "value": {"shortDescription": [{"value": "MJ", "lang": "en"}], "type": "unit group data set", "refObjectId": "93a60a57-a3c8-11da-a746-0800200c9a66", "version": "03.00.000", "uri": "../unitgroups/93a60a57-a3c8-11da-a746-0800200c9a66.xml"}}]}, "flowProperties": [], "typeOfFlow": "Other flow", "classification": {"classHierarchy": "Quantities", "name": "GaBiCategories"}}, {"dataSetInternalID": 6, "referenceToFlowDataSet": {"shortDescription": [{"value": "Use of non renewable primary energy resources used as raw materials (PENRM)", "lang": "en"}, {"value": "Nicht-erneuerbare Primärenergie zur stofflichen Nutzung (PENRM)", "lang": "de"}, {"value": "Uso de la energía primaria no renovable utilizada como materia prima (PENRM)", "lang": "es"}], "type": "flow data set", "refObjectId": "1421caa0-679d-4bf4-b282-0eb850ccae27", "version": "38.00.000", "uri": "../flows/1421caa0-679d-4bf4-b282-0eb850ccae27.xml"}, "exchange direction": "INPUT", "meanAmount": 0.0, "other": {"anies": [{"value": "224.81853025532763", "module": "A1-A3"}, {"value": "0.0", "module": "A4"}, {"value": "-3.05853025532761", "module": "A5"}, {"value": "0.0", "module": "B1"}, {"value": "0.0", "module": "B2"}, {"value": "0.0", "module": "B3"}, {"value": "0.0", "module": "B4"}, {"value": "0.0", "module": "B5"}, {"value": "0.0", "module": "B6"}, {"value": "0.0", "module": "B7"}, {"value": "0.0", "module": "C1", "scenario": "Energierückgewinnung"}, {"value": "0.0", "module": "C2", "scenario": "Energierückgewinnung"}, {"value": "-221.76000000000002", "module": "C3", "scenario": "Energierückgewinnung"}, {"value": "0.0", "module": "C4", "scenario": "Energierückgewinnung"}, {"value": "0.0", "module": "D", "scenario": "Energierückgewinnung"}, {"value": "0.0", "module": "C1", "scenario": "Recycling"}, {"value": "0.0", "module": "C2", "scenario": "Recycling"}, {"value": "-221.76000000000002", "module": "C3", "scenario": "Recycling"}, {"value": "0.0", "module": "C4", "scenario": "Recycling"}, {"value": "0.0", "module": "D", "scenario": "Recycling"}, {"name": "referenceToUnitGroupDataSet", "value": {"shortDescription": [{"value": "MJ", "lang": "en"}], "type": "unit group data set", "refObjectId": "93a60a57-a3c8-11da-a746-0800200c9a66", "version": "03.00.000", "uri": "../unitgroups/93a60a57-a3c8-11da-a746-0800200c9a66.xml"}}]}, "flowProperties": [], "typeOfFlow": "Other flow", "classification": {"classHierarchy": "Quantities", "name": "GaBiCategories"}}, {"dataSetInternalID": 7, "referenceToFlowDataSet": {"shortDescription": [{"value": "Total use of non-renewable primary energy resources (PENRT)", "lang": "en"}, {"value": "Total nicht erneuerbare Primärenergie (PENRT)", "lang": "de"}, {"value": "Uso total de la energía primaria no renovable (energía primaria y recursos de energía primaria renovable utilizada como materia prima) (PENRT)", "lang": "es"}], "type": "flow data set", "refObjectId": "06159210-646b-4c8d-8583-da9b3b95a6c1", "version": "30.00.000", "uri": "../flows/06159210-646b-4c8d-8583-da9b3b95a6c1.xml"}, "exchange direction": "INPUT", "meanAmount": 0.0, "other": {"anies": [{"value": "2707.804783268942", "module": "A1-A3"}, {"value": "210.78798473269012", "module": "A4"}, {"value": "41.60079554925755", "module": "A5"}, {"value": "0.0", "module": "B1"}, {"value": "0.0", "module": "B2"}, {"value": "0.0", "module": "B3"}, {"value": "0.0", "module": "B4"}, {"value": "0.0", "module": "B5"}, {"value": "0.0", "module": "B6"}, {"value": "0.0", "module": "B7"}, {"value": "0.0", "module": "C1", "scenario": "Energierückgewinnung"}, {"value": "64.85784145621224", "module": "C2", "scenario": "Energierückgewinnung"}, {"value": "86.60047208873252", "module": "C3", "scenario": "Energierückgewinnung"}, {"value": "0.0", "module": "C4", "scenario": "Energierückgewinnung"}, {"value": "-1910.6864396612325", "module": "D", "scenario": "Energierückgewinnung"}, {"value": "0.0", "module": "C1", "scenario": "Recycling"}, {"value": "64.85784145621224", "module": "C2", "scenario": "Recycling"}, {"value": "-2.904012287504031", "module": "C3", "scenario": "Recycling"}, {"value": "0.0", "module": "C4", "scenario": "Recycling"}, {"value": "-95.19281208508585", "module": "D", "scenario": "Recycling"}, {"name": "referenceToUnitGroupDataSet", "value": {"shortDescription": [{"value": "MJ", "lang": "en"}], "type": "unit group data set", "refObjectId": "93a60a57-a3c8-11da-a746-0800200c9a66", "version": "03.00.000", "uri": "../unitgroups/93a60a57-a3c8-11da-a746-0800200c9a66.xml"}}]}, "flowProperties": [], "typeOfFlow": "Other flow", "classification": {"classHierarchy": "Größen / Umweltliche Größen / EPD EN 15804 / LCI Indikatoren", "name": "GaBiCategories"}}, {"dataSetInternalID": 8, "referenceToFlowDataSet": {"shortDescription": [{"value": "Use of secondary material (SM)", "lang": "en"}, {"value": "Einsatz von Sekundärstoffen (SM)", "lang": "de"}, {"value": "Uso de materiales secundarios (SM)", "lang": "es"}], "type": "flow data set", "refObjectId": "c6a1f35f-2d09-4f54-8dfb-97e502e1ce92", "version": "30.00.000", "uri": "../flows/c6a1f35f-2d09-4f54-8dfb-97e502e1ce92.xml"}, "exchange direction": "INPUT", "meanAmount": 0.0, "other": {"anies": [{"value": "0.0", "module": "A1-A3"}, {"value": "0.0", "module": "A4"}, {"value": "0.0", "module": "A5"}, {"value": "0.0", "module": "B1"}, {"value": "0.0", "module": "B2"}, {"value": "0.0", "module": "B3"}, {"value": "0.0", "module": "B4"}, {"value": "0.0", "module": "B5"}, {"value": "0.0", "module": "B6"}, {"value": "0.0", "module": "B7"}, {"value": "0.0", "module": "C1", "scenario": "Energierückgewinnung"}, {"value": "0.0", "module": "C2", "scenario": "Energierückgewinnung"}, {"value": "0.0", "module": "C3", "scenario": "Energierückgewinnung"}, {"value": "0.0", "module": "C4", "scenario": "Energierückgewinnung"}, {"value": "0.0", "module": "D", "scenario": "Energierückgewinnung"}, {"value": "0.0", "module": "C1", "scenario": "Recycling"}, {"value": "0.0", "module": "C2", "scenario": "Recycling"}, {"value": "0.0", "module": "C3", "scenario": "Recycling"}, {"value": "0.0", "module": "C4", "scenario": "Recycling"}, {"value": "0.0", "module": "D", "scenario": "Recycling"}, {"name": "referenceToUnitGroupDataSet", "value": {"shortDescription": [{"value": "kg", "lang": "en"}], "type": "unit group data set", "refObjectId": "ad38d542-3fe9-439d-9b95-2f5f7752acaf", "version": "30.00.000", "uri": "../unitgroups/ad38d542-3fe9-439d-9b95-2f5f7752acaf.xml"}}]}, "flowProperties": [], "typeOfFlow": "Other flow", "classification": {"classHierarchy": "Größen / Umweltliche Größen / EPD EN 15804 / LCI Indikatoren", "name": "GaBiCategories"}}, {"dataSetInternalID": 9, "referenceToFlowDataSet": {"shortDescription": [{"value": "Use of renewable secondary fuels (RSF)", "lang": "en"}, {"value": "Erneuerbare Sekundärbrennstoffe (RSF)", "lang": "de"}, {"value": "Uso de combustibles secundarios renovables (RSF)", "lang": "es"}], "type": "flow data set", "refObjectId": "64333088-a55f-4aa2-9a31-c10b07816787", "version": "30.00.000", "uri": "../flows/64333088-a55f-4aa2-9a31-c10b07816787.xml"}, "exchange direction": "INPUT", "meanAmount": 0.0, "other": {"anies": [{"value": "0.0", "module": "A1-A3"}, {"value": "0.0", "module": "A4"}, {"value": "0.0", "module": "A5"}, {"value": "0.0", "module": "B1"}, {"value": "0.0", "module": "B2"}, {"value": "0.0", "module": "B3"}, {"value": "0.0", "module": "B4"}, {"value": "0.0", "module": "B5"}, {"value": "0.0", "module": "B6"}, {"value": "0.0", "module": "B7"}, {"value": "0.0", "module": "C1", "scenario": "Energierückgewinnung"}, {"value": "0.0", "module": "C2", "scenario": "Energierückgewinnung"}, {"value": "0.0", "module": "C3", "scenario": "Energierückgewinnung"}, {"value": "0.0", "module": "C4", "scenario": "Energierückgewinnung"}, {"value": "0.0", "module": "D", "scenario": "Energierückgewinnung"}, {"value": "0.0", "module": "C1", "scenario": "Recycling"}, {"value": "0.0", "module": "C2", "scenario": "Recycling"}, {"value": "0.0", "module": "C3", "scenario": "Recycling"}, {"value": "0.0", "module": "C4", "scenario": "Recycling"}, {"value": "0.0", "module": "D", "scenario": "Recycling"}, {"name": "referenceToUnitGroupDataSet", "value": {"shortDescription": [{"value": "MJ", "lang": "en"}], "type": "unit group data set", "refObjectId": "93a60a57-a3c8-11da-a746-0800200c9a66", "version": "03.00.000", "uri": "../unitgroups/93a60a57-a3c8-11da-a746-0800200c9a66.xml"}}]}, "flowProperties": [], "typeOfFlow": "Other flow", "classification": {"classHierarchy": "Größen / Umweltliche Größen / EPD EN 15804 / LCI Indikatoren", "name": "GaBiCategories"}}, {"dataSetInternalID": 10, "referenceToFlowDataSet": {"shortDescription": [{"value": "Use of non renewable secondary fuels (NRSF)", "lang": "en"}, {"value": "Nicht erneuerbare Sekundärbrennstoffe (NRSF)", "lang": "de"}, {"value": "Uso de combustibles secundarios no renovables (NRSF)", "lang": "es"}], "type": "flow data set", "refObjectId": "89def144-d39a-4287-b86f-efde453ddcb2", "version": "30.00.000", "uri": "../flows/89def144-d39a-4287-b86f-efde453ddcb2.xml"}, "exchange direction": "INPUT", "meanAmount": 0.0, "other": {"anies": [{"value": "0.0", "module": "A1-A3"}, {"value": "0.0", "module": "A4"}, {"value": "0.0", "module": "A5"}, {"value": "0.0", "module": "B1"}, {"value": "0.0", "module": "B2"}, {"value": "0.0", "module": "B3"}, {"value": "0.0", "module": "B4"}, {"value": "0.0", "module": "B5"}, {"value": "0.0", "module": "B6"}, {"value": "0.0", "module": "B7"}, {"value": "0.0", "module": "C1", "scenario": "Energierückgewinnung"}, {"value": "0.0", "module": "C2", "scenario": "Energierückgewinnung"}, {"value": "0.0", "module": "C3", "scenario": "Energierückgewinnung"}, {"value": "0.0", "module": "C4", "scenario": "Energierückgewinnung"}, {"value": "0.0", "module": "D", "scenario": "Energierückgewinnung"}, {"value": "0.0", "module": "C1", "scenario": "Recycling"}, {"value": "0.0", "module": "C2", "scenario": "Recycling"}, {"value": "0.0", "module": "C3", "scenario": "Recycling"}, {"value": "0.0", "module": "C4", "scenario": "Recycling"}, {"value": "0.0", "module": "D", "scenario": "Recycling"}, {"name": "referenceToUnitGroupDataSet", "value": {"shortDescription": [{"value": "MJ", "lang": "en"}], "type": "unit group data set", "refObjectId": "93a60a57-a3c8-11da-a746-0800200c9a66", "version": "03.00.000", "uri": "../unitgroups/93a60a57-a3c8-11da-a746-0800200c9a66.xml"}}]}, "flowProperties": [], "typeOfFlow": "Other flow", "classification": {"classHierarchy": "Größen / Umweltliche Größen / EPD EN 15804 / LCI Indikatoren", "name": "GaBiCategories"}}, {"dataSetInternalID": 11, "referenceToFlowDataSet": {"shortDescription": [{"value": "Use of net fresh water (FW)", "lang": "en"}, {"value": "Einsatz von Süßwasserressourcen (FW)", "lang": "de"}, {"value": "Uso neto de recursos de agua dulce (FW)", "lang": "es"}], "type": "flow data set", "refObjectId": "3cf952c8-f3a4-461d-8c96-96456ca62246", "version": "30.00.000", "uri": "../flows/3cf952c8-f3a4-461d-8c96-96456ca62246.xml"}, "exchange direction": "INPUT", "meanAmount": 0.0, "other": {"anies": [{"value": "2.4210060983041912", "module": "A1-A3"}, {"value": "0.011026308230697517", "module": "A4"}, {"value": "0.05458959932762561", "module": "A5"}, {"value": "0.0", "module": "B1"}, {"value": "0.0", "module": "B2"}, {"value": "0.0", "module": "B3"}, {"value": "0.0", "module": "B4"}, {"value": "0.0", "module": "B5"}, {"value": "0.0", "module": "B6"}, {"value": "0.0", "module": "B7"}, {"value": "0.0", "module": "C1", "scenario": "Energierückgewinnung"}, {"value": "0.003392710224830029", "module": "C2", "scenario": "Energierückgewinnung"}, {"value": "0.968151396551885", "module": "C3", "scenario": "Energierückgewinnung"}, {"value": "0.0", "module": "C4", "scenario": "Energierückgewinnung"}, {"value": "-0.41375666114657633", "module": "D", "scenario": "Energierückgewinnung"}, {"value": "0.0", "module": "C1", "scenario": "Recycling"}, {"value": "0.003392710224830029", "module": "C2", "scenario": "Recycling"}, {"value": "0.02386048224325046", "module": "C3", "scenario": "Recycling"}, {"value": "0.0", "module": "C4", "scenario": "Recycling"}, {"value": "-0.09390103066572798", "module": "D", "scenario": "Recycling"}, {"name": "referenceToUnitGroupDataSet", "value": {"shortDescription": [{"value": "m3", "lang": "en"}], "type": "unit group data set", "refObjectId": "cd950537-0a98-4044-9ba7-9f9a68d0a504", "version": "30.00.000", "uri": "../unitgroups/cd950537-0a98-4044-9ba7-9f9a68d0a504.xml"}}]}, "flowProperties": [], "typeOfFlow": "Other flow", "classification": {"classHierarchy": "Größen / Umweltliche Größen / EPD EN 15804 / LCI Indikatoren", "name": "GaBiCategories"}}, {"dataSetInternalID": 12, "referenceToFlowDataSet": {"shortDescription": [{"value": "Hazardous waste disposed (HWD)", "lang": "en"}, {"value": "Gefährlicher Abfall zur Deponie (HWD)", "lang": "de"}, {"value": "Residuos peligrosos eliminados (HWD)", "lang": "es"}], "type": "flow data set", "refObjectId": "430f9e0f-59b2-46a0-8e0d-55e0e84948fc", "version": "30.00.000", "uri": "../flows/430f9e0f-59b2-46a0-8e0d-55e0e84948fc.xml"}, "exchange direction": "OUTPUT", "meanAmount": 0.0, "other": {"anies": [{"value": "3.1335976878989604E-6", "module": "A1-A3"}, {"value": "8.9004373521118E-9", "module": "A4"}, {"value": "4.1302491203253076E-8", "module": "A5"}, {"value": "0.0", "module": "B1"}, {"value": "0.0", "module": "B2"}, {"value": "0.0", "module": "B3"}, {"value": "0.0", "module": "B4"}, {"value": "0.0", "module": "B5"}, {"value": "0.0", "module": "B6"}, {"value": "0.0", "module": "B7"}, {"value": "0.0", "module": "C1", "scenario": "Energierückgewinnung"}, {"value": "2.73859610834209E-9", "module": "C2", "scenario": "Energierückgewinnung"}, {"value": "1.56237446429491E-8", "module": "C3", "scenario": "Energierückgewinnung"}, {"value": "0.0", "module": "C4", "scenario": "Energierückgewinnung"}, {"value": "-4.290403035457638E-7", "module": "D", "scenario": "Energierückgewinnung"}, {"value": "0.0", "module": "C1", "scenario": "Recycling"}, {"value": "2.73859610834209E-9", "module": "C2", "scenario": "Recycling"}, {"value": "-1.2700824852202E-7", "module": "C3", "scenario": "Recycling"}, {"value": "0.0", "module": "C4", "scenario": "Recycling"}, {"value": "-2.1093260171073827E-8", "module": "D", "scenario": "Recycling"}, {"name": "referenceToUnitGroupDataSet", "value": {"shortDescription": [{"value": "kg", "lang": "en"}], "type": "unit group data set", "refObjectId": "ad38d542-3fe9-439d-9b95-2f5f7752acaf", "version": "30.00.000", "uri": "../unitgroups/ad38d542-3fe9-439d-9b95-2f5f7752acaf.xml"}}]}, "flowProperties": [], "typeOfFlow": "Other flow", "classification": {"classHierarchy": "Größen / Umweltliche Größen / EPD EN 15804 / LCI Indikatoren", "name": "GaBiCategories"}}, {"dataSetInternalID": 13, "referenceToFlowDataSet": {"shortDescription": [{"value": "Non-hazardous waste disposed (NHWD)", "lang": "en"}, {"value": "Entsorgter nicht gefährlicher Abfall (NHWD)", "lang": "de"}, {"value": "Residuos no peligrosos eliminados (NHWD)", "lang": "es"}], "type": "flow data set", "refObjectId": "b29ef66b-e286-4afa-949f-62f1a7b4d7fa", "version": "30.00.000", "uri": "../flows/b29ef66b-e286-4afa-949f-62f1a7b4d7fa.xml"}, "exchange direction": "OUTPUT", "meanAmount": 0.0, "other": {"anies": [{"value": "0.9266011411451146", "module": "A1-A3"}, {"value": "0.0355961410758805", "module": "A4"}, {"value": "0.11296299337975885", "module": "A5"}, {"value": "0.0", "module": "B1"}, {"value": "0.0", "module": "B2"}, {"value": "0.0", "module": "B3"}, {"value": "0.0", "module": "B4"}, {"value": "0.0", "module": "B5"}, {"value": "0.0", "module": "B6"}, {"value": "0.0", "module": "B7"}, {"value": "0.0", "module": "C1", "scenario": "Energierückgewinnung"}, {"value": "0.0109526587925786", "module": "C2", "scenario": "Energierückgewinnung"}, {"value": "2.85903118903483", "module": "C3", "scenario": "Energierückgewinnung"}, {"value": "0.0", "module": "C4", "scenario": "Energierückgewinnung"}, {"value": "-0.8906395142339528", "module": "D", "scenario": "Energierückgewinnung"}, {"value": "0.0", "module": "C1", "scenario": "Recycling"}, {"value": "0.0109526587925786", "module": "C2", "scenario": "Recycling"}, {"value": "0.0677021129970482", "module": "C3", "scenario": "Recycling"}, {"value": "0.0", "module": "C4", "scenario": "Recycling"}, {"value": "-0.29297554312719615", "module": "D", "scenario": "Recycling"}, {"name": "referenceToUnitGroupDataSet", "value": {"shortDescription": [{"value": "kg", "lang": "en"}], "type": "unit group data set", "refObjectId": "ad38d542-3fe9-439d-9b95-2f5f7752acaf", "version": "30.00.000", "uri": "../unitgroups/ad38d542-3fe9-439d-9b95-2f5f7752acaf.xml"}}]}, "flowProperties": [], "typeOfFlow": "Other flow", "classification": {"classHierarchy": "Größen / Umweltliche Größen / EPD EN 15804 / LCI Indikatoren", "name": "GaBiCategories"}}, {"dataSetInternalID": 14, "referenceToFlowDataSet": {"shortDescription": [{"value": "Radioactive waste disposed (RWD)", "lang": "en"}, {"value": "Entsorgter radioaktiver Abfall (RWD)", "lang": "de"}, {"value": "Residuos radiactivos eliminados (RWD)", "lang": "es"}], "type": "flow data set", "refObjectId": "3449546e-52ad-4b39-b809-9fb77cea8ff6", "version": "30.00.000", "uri": "../flows/3449546e-52ad-4b39-b809-9fb77cea8ff6.xml"}, "exchange direction": "OUTPUT", "meanAmount": 0.0, "other": {"anies": [{"value": "0.11301668663211979", "module": "A1-A3"}, {"value": "2.5799056780795044E-4", "module": "A4"}, {"value": "0.0015899915476938072", "module": "A5"}, {"value": "0.0", "module": "B1"}, {"value": "0.0", "module": "B2"}, {"value": "0.0", "module": "B3"}, {"value": "0.0", "module": "B4"}, {"value": "0.0", "module": "B5"}, {"value": "0.0", "module": "B6"}, {"value": "0.0", "module": "B7"}, {"value": "0.0", "module": "C1", "scenario": "Energierückgewinnung"}, {"value": "7.938171317167722E-5", "module": "C2", "scenario": "Energierückgewinnung"}, {"value": "0.004802103189240959", "module": "C3", "scenario": "Energierückgewinnung"}, {"value": "0.0", "module": "C4", "scenario": "Energierückgewinnung"}, {"value": "-0.13610291473564867", "module": "D", "scenario": "Energierückgewinnung"}, {"value": "0.0", "module": "C1", "scenario": "Recycling"}, {"value": "7.938171317167722E-5", "module": "C2", "scenario": "Recycling"}, {"value": "-0.0023280452334048986", "module": "C3", "scenario": "Recycling"}, {"value": "0.0", "module": "C4", "scenario": "Recycling"}, {"value": "-0.002606102425988038", "module": "D", "scenario": "Recycling"}, {"name": "referenceToUnitGroupDataSet", "value": {"shortDescription": [{"value": "kg", "lang": "en"}], "type": "unit group data set", "refObjectId": "ad38d542-3fe9-439d-9b95-2f5f7752acaf", "version": "30.00.000", "uri": "../unitgroups/ad38d542-3fe9-439d-9b95-2f5f7752acaf.xml"}}]}, "flowProperties": [], "typeOfFlow": "Other flow", "classification": {"classHierarchy": "Größen / Umweltliche Größen / EPD EN 15804 / LCI Indikatoren", "name": "GaBiCategories"}}, {"dataSetInternalID": 15, "referenceToFlowDataSet": {"shortDescription": [{"value": "Components for re-use (CRU)", "lang": "en"}, {"value": "Komponenten für die Wiederverwendung (CRU)", "lang": "de"}, {"value": "Componentes para su reutilización (CRU)", "lang": "es"}], "type": "flow data set", "refObjectId": "a2b32f97-3fc7-4af2-b209-525bc6426f33", "version": "30.00.000", "uri": "../flows/a2b32f97-3fc7-4af2-b209-525bc6426f33.xml"}, "exchange direction": "OUTPUT", "meanAmount": 0.0, "other": {"anies": [{"value": "0.0", "module": "A1-A3"}, {"value": "0.0", "module": "A4"}, {"value": "0.0", "module": "A5"}, {"value": "0.0", "module": "B1"}, {"value": "0.0", "module": "B2"}, {"value": "0.0", "module": "B3"}, {"value": "0.0", "module": "B4"}, {"value": "0.0", "module": "B5"}, {"value": "0.0", "module": "B6"}, {"value": "0.0", "module": "B7"}, {"value": "0.0", "module": "C1", "scenario": "Energierückgewinnung"}, {"value": "0.0", "module": "C2", "scenario": "Energierückgewinnung"}, {"value": "0.0", "module": "C3", "scenario": "Energierückgewinnung"}, {"value": "0.0", "module": "C4", "scenario": "Energierückgewinnung"}, {"value": "0.0", "module": "D", "scenario": "Energierückgewinnung"}, {"value": "0.0", "module": "C1", "scenario": "Recycling"}, {"value": "0.0", "module": "C2", "scenario": "Recycling"}, {"value": "0.0", "module": "C3", "scenario": "Recycling"}, {"value": "0.0", "module": "C4", "scenario": "Recycling"}, {"value": "0.0", "module": "D", "scenario": "Recycling"}, {"name": "referenceToUnitGroupDataSet", "value": {"shortDescription": [{"value": "kg", "lang": "en"}], "type": "unit group data set", "refObjectId": "ad38d542-3fe9-439d-9b95-2f5f7752acaf", "version": "30.00.000", "uri": "../unitgroups/ad38d542-3fe9-439d-9b95-2f5f7752acaf.xml"}}]}, "flowProperties": [], "typeOfFlow": "Other flow", "classification": {"classHierarchy": "Größen / Umweltliche Größen / EPD EN 15804 / LCI Indikatoren", "name": "GaBiCategories"}}, {"dataSetInternalID": 16, "referenceToFlowDataSet": {"shortDescription": [{"value": "Materials for recycling (MFR)", "lang": "en"}, {"value": "Stoffe zum Recycling (MFR)", "lang": "de"}, {"value": "Materiales para el reciclaje (MFR)", "lang": "es"}], "type": "flow data set", "refObjectId": "d7fe48a5-4103-49c8-9aae-b0b5dfdbd6ae", "version": "30.00.000", "uri": "../flows/d7fe48a5-4103-49c8-9aae-b0b5dfdbd6ae.xml"}, "exchange direction": "OUTPUT", "meanAmount": 0.0, "other": {"anies": [{"value": "0.0", "module": "A1-A3"}, {"value": "0.0", "module": "A4"}, {"value": "0.0", "module": "A5"}, {"value": "0.0", "module": "B1"}, {"value": "0.0", "module": "B2"}, {"value": "0.0", "module": "B3"}, {"value": "0.0", "module": "B4"}, {"value": "0.0", "module": "B5"}, {"value": "0.0", "module": "B6"}, {"value": "0.0", "module": "B7"}, {"value": "0.0", "module": "C1", "scenario": "Energierückgewinnung"}, {"value": "0.0", "module": "C2", "scenario": "Energierückgewinnung"}, {"value": "0.0", "module": "C3", "scenario": "Energierückgewinnung"}, {"value": "0.0", "module": "C4", "scenario": "Energierückgewinnung"}, {"value": "0.0", "module": "D", "scenario": "Energierückgewinnung"}, {"value": "0.0", "module": "C1", "scenario": "Recycling"}, {"value": "0.0", "module": "C2", "scenario": "Recycling"}, {"value": "0.0", "module": "C3", "scenario": "Recycling"}, {"value": "0.0", "module": "C4", "scenario": "Recycling"}, {"value": "0.0", "module": "D", "scenario": "Recycling"}, {"name": "referenceToUnitGroupDataSet", "value": {"shortDescription": [{"value": "kg", "lang": "en"}], "type": "unit group data set", "refObjectId": "ad38d542-3fe9-439d-9b95-2f5f7752acaf", "version": "30.00.000", "uri": "../unitgroups/ad38d542-3fe9-439d-9b95-2f5f7752acaf.xml"}}]}, "flowProperties": [], "typeOfFlow": "Other flow", "classification": {"classHierarchy": "Größen / Umweltliche Größen / EPD EN 15804 / LCI Indikatoren", "name": "GaBiCategories"}}, {"dataSetInternalID": 17, "referenceToFlowDataSet": {"shortDescription": [{"value": "Materials for energy recovery (MER)", "lang": "en"}, {"value": "Stoffe für die Energierückgewinnung (MER)", "lang": "de"}, {"value": "Materiales para valorización energética (recuperación de energía) (MER)", "lang": "es"}], "type": "flow data set", "refObjectId": "59a9181c-3aaf-46ee-8b13-2b3723b6e447", "version": "30.00.000", "uri": "../flows/59a9181c-3aaf-46ee-8b13-2b3723b6e447.xml"}, "exchange direction": "OUTPUT", "meanAmount": 0.0, "other": {"anies": [{"value": "0.0", "module": "A1-A3"}, {"value": "0.0", "module": "A4"}, {"value": "0.0", "module": "A5"}, {"value": "0.0", "module": "B1"}, {"value": "0.0", "module": "B2"}, {"value": "0.0", "module": "B3"}, {"value": "0.0", "module": "B4"}, {"value": "0.0", "module": "B5"}, {"value": "0.0", "module": "B6"}, {"value": "0.0", "module": "B7"}, {"value": "0.0", "module": "C1", "scenario": "Energierückgewinnung"}, {"value": "0.0", "module": "C2", "scenario": "Energierückgewinnung"}, {"value": "0.0", "module": "C3", "scenario": "Energierückgewinnung"}, {"value": "0.0", "module": "C4", "scenario": "Energierückgewinnung"}, {"value": "0.0", "module": "D", "scenario": "Energierückgewinnung"}, {"value": "0.0", "module": "C1", "scenario": "Recycling"}, {"value": "0.0", "module": "C2", "scenario": "Recycling"}, {"value": "0.0", "module": "C3", "scenario": "Recycling"}, {"value": "0.0", "module": "C4", "scenario": "Recycling"}, {"value": "0.0", "module": "D", "scenario": "Recycling"}, {"name": "referenceToUnitGroupDataSet", "value": {"shortDescription": [{"value": "kg", "lang": "en"}], "type": "unit group data set", "refObjectId": "ad38d542-3fe9-439d-9b95-2f5f7752acaf", "version": "30.00.000", "uri": "../unitgroups/ad38d542-3fe9-439d-9b95-2f5f7752acaf.xml"}}]}, "flowProperties": [], "typeOfFlow": "Other flow", "classification": {"classHierarchy": "Größen / Umweltliche Größen / EPD EN 15804 / LCI Indikatoren", "name": "GaBiCategories"}}, {"dataSetInternalID": 18, "referenceToFlowDataSet": {"shortDescription": [{"value": "Exported electrical energy (EEE)", "lang": "en"}, {"value": "Exportierte elektrische Energie (EEE)", "lang": "de"}, {"value": "Energía exportada electrica (EEE)", "lang": "es"}], "type": "flow data set", "refObjectId": "4da0c987-2b76-40d6-9e9e-82a017aaaf29", "version": "30.00.000", "uri": "../flows/4da0c987-2b76-40d6-9e9e-82a017aaaf29.xml"}, "exchange direction": "OUTPUT", "meanAmount": 0.0, "other": {"anies": [{"value": "0.0", "module": "A1-A3"}, {"value": "0.0", "module": "A4"}, {"value": "6.23562643764541", "module": "A5"}, {"value": "0.0", "module": "B1"}, {"value": "0.0", "module": "B2"}, {"value": "0.0", "module": "B3"}, {"value": "0.0", "module": "B4"}, {"value": "0.0", "module": "B5"}, {"value": "0.0", "module": "B6"}, {"value": "0.0", "module": "B7"}, {"value": "0.0", "module": "C1", "scenario": "Energierückgewinnung"}, {"value": "0.0", "module": "C2", "scenario": "Energierückgewinnung"}, {"value": "479.66357212657", "module": "C3", "scenario": "Energierückgewinnung"}, {"value": "0.0", "module": "C4", "scenario": "Energierückgewinnung"}, {"value": "0.0", "module": "D", "scenario": "Energierückgewinnung"}, {"value": "0.0", "module": "C1", "scenario": "Recycling"}, {"value": "0.0", "module": "C2", "scenario": "Recycling"}, {"value": "0.0", "module": "C3", "scenario": "Recycling"}, {"value": "0.0", "module": "C4", "scenario": "Recycling"}, {"value": "0.0", "module": "D", "scenario": "Recycling"}, {"name": "referenceToUnitGroupDataSet", "value": {"shortDescription": [{"value": "MJ", "lang": "en"}], "type": "unit group data set", "refObjectId": "93a60a57-a3c8-11da-a746-0800200c9a66", "version": "03.00.000", "uri": "../unitgroups/93a60a57-a3c8-11da-a746-0800200c9a66.xml"}}]}, "flowProperties": [], "typeOfFlow": "Other flow", "classification": {"classHierarchy": "Größen / Umweltliche Größen / EPD EN 15804 / LCI Indikatoren", "name": "GaBiCategories"}}, {"dataSetInternalID": 19, "referenceToFlowDataSet": {"shortDescription": [{"value": "Exported thermal energy (EET)", "lang": "en"}, {"value": "Exportierte thermische Energie (EET)", "lang": "de"}, {"value": "Energía exportada termal (EET)", "lang": "es"}], "type": "flow data set", "refObjectId": "98daf38a-7a79-46d3-9a37-2b7bd0955810", "version": "30.00.000", "uri": "../flows/98daf38a-7a79-46d3-9a37-2b7bd0955810.xml"}, "exchange direction": "OUTPUT", "meanAmount": 0.0, "other": {"anies": [{"value": "0.0", "module": "A1-A3"}, {"value": "0.0", "module": "A4"}, {"value": "11.1992608804867", "module": "A5"}, {"value": "0.0", "module": "B1"}, {"value": "0.0", "module": "B2"}, {"value": "0.0", "module": "B3"}, {"value": "0.0", "module": "B4"}, {"value": "0.0", "module": "B5"}, {"value": "0.0", "module": "B6"}, {"value": "0.0", "module": "B7"}, {"value": "0.0", "module": "C1", "scenario": "Energierückgewinnung"}, {"value": "0.0", "module": "C2", "scenario": "Energierückgewinnung"}, {"value": "861.481606191285", "module": "C3", "scenario": "Energierückgewinnung"}, {"value": "0.0", "module": "C4", "scenario": "Energierückgewinnung"}, {"value": "0.0", "module": "D", "scenario": "Energierückgewinnung"}, {"value": "0.0", "module": "C1", "scenario": "Recycling"}, {"value": "0.0", "module": "C2", "scenario": "Recycling"}, {"value": "0.0", "module": "C3", "scenario": "Recycling"}, {"value": "0.0", "module": "C4", "scenario": "Recycling"}, {"value": "0.0", "module": "D", "scenario": "Recycling"}, {"name": "referenceToUnitGroupDataSet", "value": {"shortDescription": [{"value": "MJ", "lang": "en"}], "type": "unit group data set", "refObjectId": "93a60a57-a3c8-11da-a746-0800200c9a66", "version": "03.00.000", "uri": "../unitgroups/93a60a57-a3c8-11da-a746-0800200c9a66.xml"}}]}, "flowProperties": [], "typeOfFlow": "Other flow", "classification": {"classHierarchy": "Größen / Umweltliche Größen / EPD EN 15804 / LCI Indikatoren", "name": "GaBiCategories"}}]}, "LCIAResults": {"LCIAResult": [{"referenceToLCIAMethodDataSet": {"shortDescription": [{"value": "Global Warming Potential - total (GWP-total)", "lang": "en"}, {"value": "Globales Erwärmungspotenzial - total (GWP-total)", "lang": "de"}], "type": "LCIA method data set", "refObjectId": "6a37f984-a4b3-458a-a20a-64418c145fa2", "version": "04.00.017", "uri": "../lciamethods/6a37f984-a4b3-458a-a20a-64418c145fa2.xml"}, "meanAmount": 0.0, "other": {"anies": [{"value": "-115.14906287273803", "module": "A1-A3"}, {"value": "15.788960696857583", "module": "A4"}, {"value": "6.07883137468294", "module": "A5"}, {"value": "0.0", "module": "B1"}, {"value": "0.0", "module": "B2"}, {"value": "0.0", "module": "B3"}, {"value": "0.0", "module": "B4"}, {"value": "0.0", "module": "B5"}, {"value": "0.0", "module": "B6"}, {"value": "0.0", "module": "B7"}, {"value": "0.0", "module": "C1", "scenario": "Energierückgewinnung"}, {"value": "4.858141752879255", "module": "C2", "scenario": "Energierückgewinnung"}, {"value": "277.2836742728735", "module": "C3", "scenario": "Energierückgewinnung"}, {"value": "0.0", "module": "C4", "scenario": "Energierückgewinnung"}, {"value": "-110.32213086665446", "module": "D", "scenario": "Energierückgewinnung"}, {"value": "0.0", "module": "C1", "scenario": "Recycling"}, {"value": "4.858141752879255", "module": "C2", "scenario": "Recycling"}, {"value": "286.4609894416472", "module": "C3", "scenario": "Recycling"}, {"value": "0.0", "module": "C4", "scenario": "Recycling"}, {"value": "-0.45443613562385954", "module": "D", "scenario": "Recycling"}, {"name": "referenceToUnitGroupDataSet", "value": {"shortDescription": [{"value": "kg CO2-eq.", "lang": "en"}], "type": "unit group data set", "refObjectId": "1ebf3012-d0db-4de2-aefd-ef30cedb0be1", "version": "30.00.000", "uri": "../unitgroups/1ebf3012-d0db-4de2-aefd-ef30cedb0be1.xml"}}]}}, {"referenceToLCIAMethodDataSet": {"shortDescription": [{"value": "Global Warming Potential - fossil fuels (GWP-fossil)", "lang": "en"}, {"value": "Globales Erwärmungspotenzial - fossil (GWP-fossil)", "lang": "de"}], "type": "LCIA method data set", "refObjectId": "5f635281-343e-44fb-83df-1971b155e6b6", "version": "01.00.009", "uri": "../lciamethods/5f635281-343e-44fb-83df-1971b155e6b6.xml"}, "meanAmount": 0.0, "other": {"anies": [{"value": "159.48366146412914", "module": "A1-A3"}, {"value": "15.687108938803574", "module": "A4"}, {"value": "2.670128531861719", "module": "A5"}, {"value": "0.0", "module": "B1"}, {"value": "0.0", "module": "B2"}, {"value": "0.0", "module": "B3"}, {"value": "0.0", "module": "B4"}, {"value": "0.0", "module": "B5"}, {"value": "0.0", "module": "B6"}, {"value": "0.0", "module": "B7"}, {"value": "0.0", "module": "C1", "scenario": "Energierückgewinnung"}, {"value": "4.826802750401098", "module": "C2", "scenario": "Energierückgewinnung"}, {"value": "5.880002446703257", "module": "C3", "scenario": "Energierückgewinnung"}, {"value": "0.0", "module": "C4", "scenario": "Energierückgewinnung"}, {"value": "-110.24679678574185", "module": "D", "scenario": "Energierückgewinnung"}, {"value": "0.0", "module": "C1", "scenario": "Recycling"}, {"value": "4.826802750401098", "module": "C2", "scenario": "Recycling"}, {"value": "15.058953681228271", "module": "C3", "scenario": "Recycling"}, {"value": "0.0", "module": "C4", "scenario": "Recycling"}, {"value": "-0.422184080975325", "module": "D", "scenario": "Recycling"}, {"name": "referenceToUnitGroupDataSet", "value": {"shortDescription": [{"value": "kg CO2-eq.", "lang": "en"}], "type": "unit group data set", "refObjectId": "1ebf3012-d0db-4de2-aefd-ef30cedb0be1", "version": "30.00.000", "uri": "../unitgroups/1ebf3012-d0db-4de2-aefd-ef30cedb0be1.xml"}}]}}, {"referenceToLCIAMethodDataSet": {"shortDescription": [{"value": "Global Warming Potential - biogenic (GWP-biogenic)", "lang": "en"}, {"value": "Globales Erwärmungspotenzial - biogen (GWP-biogenic)", "lang": "de"}], "type": "LCIA method data set", "refObjectId": "2356e1ab-0185-4db5-86e5-16de51c7485c", "version": "01.00.006", "uri": "../lciamethods/2356e1ab-0185-4db5-86e5-16de51c7485c.xml"}, "meanAmount": 0.0, "other": {"anies": [{"value": "-274.8042077054357", "module": "A1-A3"}, {"value": "0.0", "module": "A4"}, {"value": "3.40431026953827", "module": "A5"}, {"value": "0.0", "module": "B1"}, {"value": "0.0", "module": "B2"}, {"value": "0.0", "module": "B3"}, {"value": "0.0", "module": "B4"}, {"value": "0.0", "module": "B5"}, {"value": "0.0", "module": "B6"}, {"value": "0.0", "module": "B7"}, {"value": "0.0", "module": "C1", "scenario": "Energierückgewinnung"}, {"value": "0.0", "module": "C2", "scenario": "Energierückgewinnung"}, {"value": "271.39989743589746", "module": "C3", "scenario": "Energierückgewinnung"}, {"value": "0.0", "module": "C4", "scenario": "Energierückgewinnung"}, {"value": "0.0", "module": "D", "scenario": "Energierückgewinnung"}, {"value": "0.0", "module": "C1", "scenario": "Recycling"}, {"value": "0.0", "module": "C2", "scenario": "Recycling"}, {"value": "271.39989743589746", "module": "C3", "scenario": "Recycling"}, {"value": "0.0", "module": "C4", "scenario": "Recycling"}, {"value": "0.0", "module": "D", "scenario": "Recycling"}, {"name": "referenceToUnitGroupDataSet", "value": {"shortDescription": [{"value": "kg CO2-eq.", "lang": "en"}], "type": "unit group data set", "refObjectId": "1ebf3012-d0db-4de2-aefd-ef30cedb0be1", "version": "30.00.000", "uri": "../unitgroups/1ebf3012-d0db-4de2-aefd-ef30cedb0be1.xml"}}]}}, {"referenceToLCIAMethodDataSet": {"shortDescription": [{"value": "Global Warming Potential - land use and land use change (GWP-luluc)", "lang": "en"}, {"value": "Globales Erwärmungspotenzial - luluc (GWP-luluc)", "lang": "de"}], "type": "LCIA method data set", "refObjectId": "4331bbdb-978a-490d-8707-eeb047f01a55", "version": "01.00.006", "uri": "../lciamethods/4331bbdb-978a-490d-8707-eeb047f01a55.xml"}, "meanAmount": 0.0, "other": {"anies": [{"value": "0.17148336856853796", "module": "A1-A3"}, {"value": "0.1018517580540084", "module": "A4"}, {"value": "0.004392573282951236", "module": "A5"}, {"value": "0.0", "module": "B1"}, {"value": "0.0", "module": "B2"}, {"value": "0.0", "module": "B3"}, {"value": "0.0", "module": "B4"}, {"value": "0.0", "module": "B5"}, {"value": "0.0", "module": "B6"}, {"value": "0.0", "module": "B7"}, {"value": "0.0", "module": "C1", "scenario": "Energierückgewinnung"}, {"value": "0.03133900247815653", "module": "C2", "scenario": "Energierückgewinnung"}, {"value": "0.0037743902727779967", "module": "C3", "scenario": "Energierückgewinnung"}, {"value": "0.0", "module": "C4", "scenario": "Energierückgewinnung"}, {"value": "-0.07533408091261472", "module": "D", "scenario": "Energierückgewinnung"}, {"value": "0.0", "module": "C1", "scenario": "Recycling"}, {"value": "0.03133900247815653", "module": "C2", "scenario": "Recycling"}, {"value": "0.0021383245214439597", "module": "C3", "scenario": "Recycling"}, {"value": "0.0", "module": "C4", "scenario": "Recycling"}, {"value": "-0.03225205464853454", "module": "D", "scenario": "Recycling"}, {"name": "referenceToUnitGroupDataSet", "value": {"shortDescription": [{"value": "kg CO2-eq.", "lang": "en"}], "type": "unit group data set", "refObjectId": "1ebf3012-d0db-4de2-aefd-ef30cedb0be1", "version": "30.00.000", "uri": "../unitgroups/1ebf3012-d0db-4de2-aefd-ef30cedb0be1.xml"}}]}}, {"referenceToLCIAMethodDataSet": {"shortDescription": [{"value": "Depletion potential of the stratospheric ozone layer (ODP)", "lang": "en"}, {"value": "Abbaupotenzial der stratosphärischen Ozonschicht (ODP)", "lang": "de"}], "type": "LCIA method data set", "refObjectId": "b5c629d6-def3-11e6-bf01-fe55135034f3", "version": "02.00.013", "uri": "../lciamethods/b5c629d6-def3-11e6-bf01-fe55135034f3.xml"}, "meanAmount": 0.0, "other": {"anies": [{"value": "1.743885213118084E-5", "module": "A1-A3"}, {"value": "5.64321423054415E-15", "module": "A4"}, {"value": "2.267050790998358E-7", "module": "A5"}, {"value": "0.0", "module": "B1"}, {"value": "0.0", "module": "B2"}, {"value": "0.0", "module": "B3"}, {"value": "0.0", "module": "B4"}, {"value": "0.0", "module": "B5"}, {"value": "0.0", "module": "B6"}, {"value": "0.0", "module": "B7"}, {"value": "0.0", "module": "C1", "scenario": "Energierückgewinnung"}, {"value": "1.7363736093981975E-15", "module": "C2", "scenario": "Energierückgewinnung"}, {"value": "5.218338695963157E-14", "module": "C3", "scenario": "Energierückgewinnung"}, {"value": "0.0", "module": "C4", "scenario": "Energierückgewinnung"}, {"value": "-1.2394018820924802E-12", "module": "D", "scenario": "Energierückgewinnung"}, {"value": "0.0", "module": "C1", "scenario": "Recycling"}, {"value": "1.7363736093981975E-15", "module": "C2", "scenario": "Recycling"}, {"value": "-7.18679814401856E-14", "module": "C3", "scenario": "Recycling"}, {"value": "0.0", "module": "C4", "scenario": "Recycling"}, {"value": "-3.8270518032690717E-14", "module": "D", "scenario": "Recycling"}, {"name": "referenceToUnitGroupDataSet", "value": {"shortDescription": [{"value": "kg CFC-11-eq.", "lang": "en"}], "type": "unit group data set", "refObjectId": "d9e957c9-7309-4474-bf3a-7777df6c4e5b", "version": "25.00.000", "uri": "../unitgroups/d9e957c9-7309-4474-bf3a-7777df6c4e5b.xml"}}]}}, {"referenceToLCIAMethodDataSet": {"shortDescription": [{"value": "Acidification potential, Accumulated Exceedance (AP)", "lang": "en"}, {"value": "Versauerungspotenzial, kumulierte Überschreitung (AP)", "lang": "de"}], "type": "LCIA method data set", "refObjectId": "b5c611c6-def3-11e6-bf01-fe55135034f3", "version": "01.03.010", "uri": "../lciamethods/b5c611c6-def3-11e6-bf01-fe55135034f3.xml"}, "meanAmount": 0.0, "other": {"anies": [{"value": "0.8505091111862023", "module": "A1-A3"}, {"value": "0.08278999218442784", "module": "A4"}, {"value": "0.014226223706182898", "module": "A5"}, {"value": "0.0", "module": "B1"}, {"value": "0.0", "module": "B2"}, {"value": "0.0", "module": "B3"}, {"value": "0.0", "module": "B4"}, {"value": "0.0", "module": "B5"}, {"value": "0.0", "module": "B6"}, {"value": "0.0", "module": "B7"}, {"value": "0.0", "module": "C1", "scenario": "Energierückgewinnung"}, {"value": "0.025473843749054682", "module": "C2", "scenario": "Energierückgewinnung"}, {"value": "0.05660168549837948", "module": "C3", "scenario": "Energierückgewinnung"}, {"value": "0.0", "module": "C4", "scenario": "Energierückgewinnung"}, {"value": "-0.14246189464328649", "module": "D", "scenario": "Energierückgewinnung"}, {"value": "0.0", "module": "C1", "scenario": "Recycling"}, {"value": "0.025473843749054682", "module": "C2", "scenario": "Recycling"}, {"value": "0.3112397063404383", "module": "C3", "scenario": "Recycling"}, {"value": "0.0", "module": "C4", "scenario": "Recycling"}, {"value": "-0.19856174882376992", "module": "D", "scenario": "Recycling"}, {"name": "referenceToUnitGroupDataSet", "value": {"shortDescription": [{"value": "mol H+-eq.", "lang": "en"}], "type": "unit group data set", "refObjectId": "42e089ac-92bf-4bf2-8ca1-5fc40d18f2ed", "version": "00.01.000", "uri": "../unitgroups/42e089ac-92bf-4bf2-8ca1-5fc40d18f2ed.xml"}}]}}, {"referenceToLCIAMethodDataSet": {"shortDescription": [{"value": "Eutrophication potential - freshwater (EP-freshwater)", "lang": "en"}, {"value": "Eutrophierungspotenzial - Süßwasser (EP-freshwater)", "lang": "de"}], "type": "LCIA method data set", "refObjectId": "b53ec18f-7377-4ad3-86eb-cc3f4f276b2b", "version": "01.00.011", "uri": "../lciamethods/b53ec18f-7377-4ad3-86eb-cc3f4f276b2b.xml"}, "meanAmount": 0.0, "other": {"anies": [{"value": "0.026927501544430087", "module": "A1-A3"}, {"value": "3.2955439878303404E-5", "module": "A4"}, {"value": "3.509136852297382E-4", "module": "A5"}, {"value": "0.0", "module": "B1"}, {"value": "0.0", "module": "B2"}, {"value": "0.0", "module": "B3"}, {"value": "0.0", "module": "B4"}, {"value": "0.0", "module": "B5"}, {"value": "0.0", "module": "B6"}, {"value": "0.0", "module": "B7"}, {"value": "0.0", "module": "C1", "scenario": "Energierückgewinnung"}, {"value": "1.0140135347170272E-5", "module": "C2", "scenario": "Energierückgewinnung"}, {"value": "7.153023723124939E-6", "module": "C3", "scenario": "Energierückgewinnung"}, {"value": "0.0", "module": "C4", "scenario": "Energierückgewinnung"}, {"value": "-1.4237351401033996E-4", "module": "D", "scenario": "Energierückgewinnung"}, {"value": "0.0", "module": "C1", "scenario": "Recycling"}, {"value": "1.0140135347170272E-5", "module": "C2", "scenario": "Recycling"}, {"value": "-1.0320057920674923E-4", "module": "C3", "scenario": "Recycling"}, {"value": "0.0", "module": "C4", "scenario": "Recycling"}, {"value": "-6.494723923064614E-4", "module": "D", "scenario": "Recycling"}, {"name": "referenceToUnitGroupDataSet", "value": {"shortDescription": [{"value": "kg P-eq.", "lang": "en"}], "type": "unit group data set", "refObjectId": "0429039d-a61d-4590-ba67-aa4a20a810a1", "version": "30.00.000", "uri": "../unitgroups/0429039d-a61d-4590-ba67-aa4a20a810a1.xml"}}]}}, {"referenceToLCIAMethodDataSet": {"shortDescription": [{"value": "Eutrophication potential - marine (EP-marine)", "lang": "en"}, {"value": "Eutrophierungspotenzial - Salzwasser (EP-marine)", "lang": "de"}], "type": "LCIA method data set", "refObjectId": "b5c619fa-def3-11e6-bf01-fe55135034f3", "version": "02.00.011", "uri": "../lciamethods/b5c619fa-def3-11e6-bf01-fe55135034f3.xml"}, "meanAmount": 0.0, "other": {"anies": [{"value": "0.5074576074302891", "module": "A1-A3"}, {"value": "0.04041785537686868", "module": "A4"}, {"value": "0.00791897673928001", "module": "A5"}, {"value": "0.0", "module": "B1"}, {"value": "0.0", "module": "B2"}, {"value": "0.0", "module": "B3"}, {"value": "0.0", "module": "B4"}, {"value": "0.0", "module": "B5"}, {"value": "0.0", "module": "B6"}, {"value": "0.0", "module": "B7"}, {"value": "0.0", "module": "C1", "scenario": "Energierückgewinnung"}, {"value": "0.01243626319288271", "module": "C2", "scenario": "Energierückgewinnung"}, {"value": "0.01859283353601945", "module": "C3", "scenario": "Energierückgewinnung"}, {"value": "0.0", "module": "C4", "scenario": "Energierückgewinnung"}, {"value": "-0.040714740671187404", "module": "D", "scenario": "Energierückgewinnung"}, {"value": "0.0", "module": "C1", "scenario": "Recycling"}, {"value": "0.01243626319288271", "module": "C2", "scenario": "Recycling"}, {"value": "0.008139331037847638", "module": "C3", "scenario": "Recycling"}, {"value": "0.0", "module": "C4", "scenario": "Recycling"}, {"value": "-0.014521397446962367", "module": "D", "scenario": "Recycling"}, {"name": "referenceToUnitGroupDataSet", "value": {"shortDescription": [{"value": "kg N-eq.", "lang": "en"}], "type": "unit group data set", "refObjectId": "d05bb823-ecdf-4686-8c40-bf1d9257859f", "version": "00.00.003", "uri": "../unitgroups/d05bb823-ecdf-4686-8c40-bf1d9257859f.xml"}}]}}, {"referenceToLCIAMethodDataSet": {"shortDescription": [{"value": "Eutrophication potential - terrestrial (EP-terrestrial)", "lang": "en"}, {"value": "Eutrophierungspotenzial - Land (EP-terrestrial)", "lang": "de"}], "type": "LCIA method data set", "refObjectId": "b5c614d2-def3-11e6-bf01-fe55135034f3", "version": "01.02.010", "uri": "../lciamethods/b5c614d2-def3-11e6-bf01-fe55135034f3.xml"}, "meanAmount": 0.0, "other": {"anies": [{"value": "3.014381328548447", "module": "A1-A3"}, {"value": "0.4481504393841249", "module": "A4"}, {"value": "0.055287209185504366", "module": "A5"}, {"value": "0.0", "module": "B1"}, {"value": "0.0", "module": "B2"}, {"value": "0.0", "module": "B3"}, {"value": "0.0", "module": "B4"}, {"value": "0.0", "module": "B5"}, {"value": "0.0", "module": "B6"}, {"value": "0.0", "module": "B7"}, {"value": "0.0", "module": "C1", "scenario": "Energierückgewinnung"}, {"value": "0.13789244288742275", "module": "C2", "scenario": "Energierückgewinnung"}, {"value": "0.26979728641226125", "module": "C3", "scenario": "Energierückgewinnung"}, {"value": "0.0", "module": "C4", "scenario": "Energierückgewinnung"}, {"value": "-0.43633558436182424", "module": "D", "scenario": "Energierückgewinnung"}, {"value": "0.0", "module": "C1", "scenario": "Recycling"}, {"value": "0.13789244288742275", "module": "C2", "scenario": "Recycling"}, {"value": "1.4166420514552447", "module": "C3", "scenario": "Recycling"}, {"value": "0.0", "module": "C4", "scenario": "Recycling"}, {"value": "-0.8639974003735961", "module": "D", "scenario": "Recycling"}, {"name": "referenceToUnitGroupDataSet", "value": {"shortDescription": [{"value": "mol N-eq.", "lang": "en"}], "type": "unit group data set", "refObjectId": "71b4d617-0ec9-4d3f-b65e-e438940c2401", "version": "00.00.003", "uri": "../unitgroups/71b4d617-0ec9-4d3f-b65e-e438940c2401.xml"}}]}}, {"referenceToLCIAMethodDataSet": {"shortDescription": [{"value": "Photochemical Ozone Creation Potential (POCP)", "lang": "en"}, {"value": "Bildungspotenzial für troposphärisches Ozon (POCP)", "lang": "de"}], "type": "LCIA method data set", "refObjectId": "b5c610fe-def3-11e6-bf01-fe55135034f3", "version": "02.00.015", "uri": "../lciamethods/b5c610fe-def3-11e6-bf01-fe55135034f3.xml"}, "meanAmount": 0.0, "other": {"anies": [{"value": "0.3706171685446426", "module": "A1-A3"}, {"value": "0.07814716808907489", "module": "A4"}, {"value": "0.007758220812594639", "module": "A5"}, {"value": "0.0", "module": "B1"}, {"value": "0.0", "module": "B2"}, {"value": "0.0", "module": "B3"}, {"value": "0.0", "module": "B4"}, {"value": "0.0", "module": "B5"}, {"value": "0.0", "module": "B6"}, {"value": "0.0", "module": "B7"}, {"value": "0.0", "module": "C1", "scenario": "Energierückgewinnung"}, {"value": "0.024045282488946086", "module": "C2", "scenario": "Energierückgewinnung"}, {"value": "0.05050706559699725", "module": "C3", "scenario": "Energierückgewinnung"}, {"value": "0.0", "module": "C4", "scenario": "Energierückgewinnung"}, {"value": "-0.11435760141308579", "module": "D", "scenario": "Energierückgewinnung"}, {"value": "0.0", "module": "C1", "scenario": "Recycling"}, {"value": "0.024045282488946086", "module": "C2", "scenario": "Recycling"}, {"value": "0.08299572869273854", "module": "C3", "scenario": "Recycling"}, {"value": "0.0", "module": "C4", "scenario": "Recycling"}, {"value": "0.0033105196136766057", "module": "D", "scenario": "Recycling"}, {"name": "referenceToUnitGroupDataSet", "value": {"shortDescription": [{"value": "kg NMVOC-eq.", "lang": "en"}], "type": "unit group data set", "refObjectId": "d27c25f8-fbc1-44c6-b47b-4adbae4199c6", "version": "00.00.003", "uri": "../unitgroups/d27c25f8-fbc1-44c6-b47b-4adbae4199c6.xml"}}]}}, {"referenceToLCIAMethodDataSet": {"shortDescription": [{"value": "Abiotic depletion potential - non-fossil resources (ADPE)", "lang": "en"}, {"value": "Potenzial für die Verknappung abiotischer Ressourcen – nicht fossile Ressourcen (ADPE)", "lang": "de"}], "type": "LCIA method data set", "refObjectId": "b2ad6494-c78d-11e6-9d9d-cec0c932ce01", "version": "01.00.011", "uri": "../lciamethods/b2ad6494-c78d-11e6-9d9d-cec0c932ce01.xml"}, "meanAmount": 0.0, "other": {"anies": [{"value": "0.0010216931062452966", "module": "A1-A3"}, {"value": "1.4611413702060528E-6", "module": "A4"}, {"value": "1.3331177775535319E-5", "module": "A5"}, {"value": "0.0", "module": "B1"}, {"value": "0.0", "module": "B2"}, {"value": "0.0", "module": "B3"}, {"value": "0.0", "module": "B4"}, {"value": "0.0", "module": "B5"}, {"value": "0.0", "module": "B6"}, {"value": "0.0", "module": "B7"}, {"value": "0.0", "module": "C1", "scenario": "Energierückgewinnung"}, {"value": "4.4958196006340073E-7", "module": "C2", "scenario": "Energierückgewinnung"}, {"value": "7.955338709792713E-7", "module": "C3", "scenario": "Energierückgewinnung"}, {"value": "0.0", "module": "C4", "scenario": "Energierückgewinnung"}, {"value": "-1.812979622088984E-5", "module": "D", "scenario": "Energierückgewinnung"}, {"value": "0.0", "module": "C1", "scenario": "Recycling"}, {"value": "4.4958196006340073E-7", "module": "C2", "scenario": "Recycling"}, {"value": "-1.3902793377885419E-6", "module": "C3", "scenario": "Recycling"}, {"value": "0.0", "module": "C4", "scenario": "Recycling"}, {"value": "-3.557633995943312E-6", "module": "D", "scenario": "Recycling"}, {"name": "referenceToUnitGroupDataSet", "value": {"shortDescription": [{"value": "kg Sb-eq.", "lang": "en"}], "type": "unit group data set", "refObjectId": "54ccd2d9-a32a-4fc2-923d-f2c8c93e89d4", "version": "30.00.000", "uri": "../unitgroups/54ccd2d9-a32a-4fc2-923d-f2c8c93e89d4.xml"}}]}}, {"referenceToLCIAMethodDataSet": {"shortDescription": [{"value": "Abiotic depletion potential - fossil resources (ADPF)", "lang": "en"}, {"value": "Potenzial für die Verknappung abiotischer Ressourcen – fossile Brennstoffe (ADPF)", "lang": "de"}], "type": "LCIA method data set", "refObjectId": "b2ad6110-c78d-11e6-9d9d-cec0c932ce01", "version": "01.00.011", "uri": "../lciamethods/b2ad6110-c78d-11e6-9d9d-cec0c932ce01.xml"}, "meanAmount": 0.0, "other": {"anies": [{"value": "2707.10205523991", "module": "A1-A3"}, {"value": "210.68382535482235", "module": "A4"}, {"value": "41.588597461576", "module": "A5"}, {"value": "0.0", "module": "B1"}, {"value": "0.0", "module": "B2"}, {"value": "0.0", "module": "B3"}, {"value": "0.0", "module": "B4"}, {"value": "0.0", "module": "B5"}, {"value": "0.0", "module": "B6"}, {"value": "0.0", "module": "B7"}, {"value": "0.0", "module": "C1", "scenario": "Energierückgewinnung"}, {"value": "64.82579241686831", "module": "C2", "scenario": "Energierückgewinnung"}, {"value": "86.55976139410538", "module": "C3", "scenario": "Energierückgewinnung"}, {"value": "0.0", "module": "C4", "scenario": "Energierückgewinnung"}, {"value": "-1910.4591277416223", "module": "D", "scenario": "Energierückgewinnung"}, {"value": "0.0", "module": "C1", "scenario": "Recycling"}, {"value": "64.82579241686831", "module": "C2", "scenario": "Recycling"}, {"value": "-2.9187731665476635", "module": "C3", "scenario": "Recycling"}, {"value": "0.0", "module": "C4", "scenario": "Recycling"}, {"value": "-95.17477158426878", "module": "D", "scenario": "Recycling"}, {"name": "referenceToUnitGroupDataSet", "value": {"shortDescription": [{"value": "MJ", "lang": "en"}], "type": "unit group data set", "refObjectId": "93a60a57-a3c8-11da-a746-0800200c9a66", "version": "03.00.000", "uri": "../unitgroups/93a60a57-a3c8-11da-a746-0800200c9a66.xml"}}]}}, {"referenceToLCIAMethodDataSet": {"shortDescription": [{"value": "Water (user) deprivation potential (WDP)", "lang": "en"}, {"value": "Wasser-Entzugspotenzial (Benutzer) (WDP)", "lang": "de"}], "type": "LCIA method data set", "refObjectId": "b2ad66ce-c78d-11e6-9d9d-cec0c932ce01", "version": "03.00.015", "uri": "../lciamethods/b2ad66ce-c78d-11e6-9d9d-cec0c932ce01.xml"}, "meanAmount": 0.0, "other": {"anies": [{"value": "94.39193748497368", "module": "A1-A3"}, {"value": "0.0621186040153699", "module": "A4"}, {"value": "2.2017011248586686", "module": "A5"}, {"value": "0.0", "module": "B1"}, {"value": "0.0", "module": "B2"}, {"value": "0.0", "module": "B3"}, {"value": "0.0", "module": "B4"}, {"value": "0.0", "module": "B5"}, {"value": "0.0", "module": "B6"}, {"value": "0.0", "module": "B7"}, {"value": "0.0", "module": "C1", "scenario": "Energierückgewinnung"}, {"value": "0.019113416620113576", "module": "C2", "scenario": "Energierückgewinnung"}, {"value": "41.174650377068986", "module": "C3", "scenario": "Energierückgewinnung"}, {"value": "0.0", "module": "C4", "scenario": "Energierückgewinnung"}, {"value": "-8.210055379021682", "module": "D", "scenario": "Energierückgewinnung"}, {"value": "0.0", "module": "C1", "scenario": "Recycling"}, {"value": "0.019113416620113576", "module": "C2", "scenario": "Recycling"}, {"value": "2.190378147138581", "module": "C3", "scenario": "Recycling"}, {"value": "0.0", "module": "C4", "scenario": "Recycling"}, {"value": "-0.26375935137598455", "module": "D", "scenario": "Recycling"}, {"name": "referenceToUnitGroupDataSet", "value": {"shortDescription": [{"value": "m3 world eq. deprived", "lang": "en"}], "type": "unit group data set", "refObjectId": "6ae2df01-888e-46c8-b17d-49fa3869b476", "version": "00.00.003", "uri": "../unitgroups/6ae2df01-888e-46c8-b17d-49fa3869b476.xml"}}]}}, {"referenceToLCIAMethodDataSet": {"shortDescription": [{"value": "Potential incidence of disease due to PM emissions (PM)", "lang": "en"}, {"value": "Potenzielles Auftreten von Krankheiten aufgrund von Feinstaubemissionen (PM)", "lang": "de"}], "type": "LCIA method data set", "refObjectId": "b5c602c6-def3-11e6-bf01-fe55135034f3", "version": "02.00.012", "uri": "../lciamethods/b5c602c6-def3-11e6-bf01-fe55135034f3.xml"}, "meanAmount": 0.0, "other": {"anies": [{"value": "6.350487116591094E-6", "module": "A1-A3"}, {"value": "3.1605222503305895E-7", "module": "A4"}, {"value": "9.665343532237448E-8", "module": "A5"}, {"value": "0.0", "module": "B1"}, {"value": "0.0", "module": "B2"}, {"value": "0.0", "module": "B3"}, {"value": "0.0", "module": "B4"}, {"value": "0.0", "module": "B5"}, {"value": "0.0", "module": "B6"}, {"value": "0.0", "module": "B7"}, {"value": "0.0", "module": "C1", "scenario": "Energierückgewinnung"}, {"value": "9.72468384717106E-8", "module": "C2", "scenario": "Energierückgewinnung"}, {"value": "2.8378786505469807E-7", "module": "C3", "scenario": "Energierückgewinnung"}, {"value": "0.0", "module": "C4", "scenario": "Energierückgewinnung"}, {"value": "-1.2261696120367012E-6", "module": "D", "scenario": "Energierückgewinnung"}, {"value": "0.0", "module": "C1", "scenario": "Recycling"}, {"value": "9.72468384717106E-8", "module": "C2", "scenario": "Recycling"}, {"value": "2.1152327441848013E-6", "module": "C3", "scenario": "Recycling"}, {"value": "0.0", "module": "C4", "scenario": "Recycling"}, {"value": "-1.4927843260125503E-6", "module": "D", "scenario": "Recycling"}, {"name": "referenceToUnitGroupDataSet", "value": {"shortDescription": [{"value": "Disease incidence", "lang": "en"}], "type": "unit group data set", "refObjectId": "3883559b-648f-4afc-8ba2-0bd24f3affa3", "version": "00.00.003", "uri": "../unitgroups/3883559b-648f-4afc-8ba2-0bd24f3affa3.xml"}}]}}, {"referenceToLCIAMethodDataSet": {"shortDescription": [{"value": "Potential Human exposure efficiency relative to U235 (IRP)", "lang": "en"}, {"value": "Potenzielle Wirkung durch Exposition des Menschen mit U235 (IRP)", "lang": "de"}], "type": "LCIA method data set", "refObjectId": "b5c632be-def3-11e6-bf01-fe55135034f3", "version": "01.00.012", "uri": "../lciamethods/b5c632be-def3-11e6-bf01-fe55135034f3.xml"}, "meanAmount": 0.0, "other": {"anies": [{"value": "17.385214223187084", "module": "A1-A3"}, {"value": "0.02542542093560488", "module": "A4"}, {"value": "0.24476610091864245", "module": "A5"}, {"value": "0.0", "module": "B1"}, {"value": "0.0", "module": "B2"}, {"value": "0.0", "module": "B3"}, {"value": "0.0", "module": "B4"}, {"value": "0.0", "module": "B5"}, {"value": "0.0", "module": "B6"}, {"value": "0.0", "module": "B7"}, {"value": "0.0", "module": "C1", "scenario": "Energierückgewinnung"}, {"value": "0.007823206441724587", "module": "C2", "scenario": "Energierückgewinnung"}, {"value": "0.761102206359522", "module": "C3", "scenario": "Energierückgewinnung"}, {"value": "0.0", "module": "C4", "scenario": "Energierückgewinnung"}, {"value": "-22.289185796464924", "module": "D", "scenario": "Energierückgewinnung"}, {"value": "0.0", "module": "C1", "scenario": "Recycling"}, {"value": "0.007823206441724587", "module": "C2", "scenario": "Recycling"}, {"value": "-0.18426066928144627", "module": "C3", "scenario": "Recycling"}, {"value": "0.0", "module": "C4", "scenario": "Recycling"}, {"value": "-0.3836803112380693", "module": "D", "scenario": "Recycling"}, {"name": "referenceToUnitGroupDataSet", "value": {"shortDescription": [{"value": "kgBq U235-eq.", "lang": "en"}], "type": "unit group data set", "refObjectId": "456b05bf-1415-44a9-9993-02452f554c09", "version": "00.00.003", "uri": "../unitgroups/456b05bf-1415-44a9-9993-02452f554c09.xml"}}]}}, {"referenceToLCIAMethodDataSet": {"shortDescription": [{"value": "Potential Comparative Toxic Unit for ecosystems (ETP-fw)", "lang": "en"}, {"value": "Potenzielle Toxizitätsvergleichseinheit für Ökosysteme (ETP-fw)", "lang": "de"}], "type": "LCIA method data set", "refObjectId": "ee1082d1-b0f7-43ca-a1f0-21e2a4a74511", "version": "01.00.003", "uri": "../lciamethods/ee1082d1-b0f7-43ca-a1f0-21e2a4a74511.xml"}, "meanAmount": 0.0, "other": {"anies": [{"value": "5258.475534388987", "module": "A1-A3"}, {"value": "170.13113199001882", "module": "A4"}, {"value": "72.74541059661394", "module": "A5"}, {"value": "0.0", "module": "B1"}, {"value": "0.0", "module": "B2"}, {"value": "0.0", "module": "B3"}, {"value": "0.0", "module": "B4"}, {"value": "0.0", "module": "B5"}, {"value": "0.0", "module": "B6"}, {"value": "0.0", "module": "B7"}, {"value": "0.0", "module": "C1", "scenario": "Energierückgewinnung"}, {"value": "52.34804061231353", "module": "C2", "scenario": "Energierückgewinnung"}, {"value": "37.39873163412358", "module": "C3", "scenario": "Energierückgewinnung"}, {"value": "0.0", "module": "C4", "scenario": "Energierückgewinnung"}, {"value": "-392.7442846972096", "module": "D", "scenario": "Energierückgewinnung"}, {"value": "0.0", "module": "C1", "scenario": "Recycling"}, {"value": "52.34804061231353", "module": "C2", "scenario": "Recycling"}, {"value": "25.396182883793845", "module": "C3", "scenario": "Recycling"}, {"value": "0.0", "module": "C4", "scenario": "Recycling"}, {"value": "181114.57262287714", "module": "D", "scenario": "Recycling"}, {"name": "referenceToUnitGroupDataSet", "value": {"shortDescription": [{"value": "CTUe", "lang": "en"}], "type": "unit group data set", "refObjectId": "aa959ded-f1eb-4efb-9c5c-2d60be36b3e6", "version": "00.00.003", "uri": "../unitgroups/aa959ded-f1eb-4efb-9c5c-2d60be36b3e6.xml"}}]}}, {"referenceToLCIAMethodDataSet": {"shortDescription": [{"value": "Potential Comparative Toxic Unit for humans - cancer effects (HTP-c)", "lang": "en"}, {"value": "Potenzielle Toxizitätsvergleichseinheit für den Menschen - kanzerogene Wirkung (HTP-c)", "lang": "de"}], "type": "LCIA method data set", "refObjectId": "2299222a-bbd8-474f-9d4f-4dd1f18aea7c", "version": "01.00.004", "uri": "../lciamethods/2299222a-bbd8-474f-9d4f-4dd1f18aea7c.xml"}, "meanAmount": 0.0, "other": {"anies": [{"value": "1.2382957027439854E-7", "module": "A1-A3"}, {"value": "3.4156259195648796E-9", "module": "A4"}, {"value": "1.7393098344295581E-9", "module": "A5"}, {"value": "0.0", "module": "B1"}, {"value": "0.0", "module": "B2"}, {"value": "0.0", "module": "B3"}, {"value": "0.0", "module": "B4"}, {"value": "0.0", "module": "B5"}, {"value": "0.0", "module": "B6"}, {"value": "0.0", "module": "B7"}, {"value": "0.0", "module": "C1", "scenario": "Energierückgewinnung"}, {"value": "1.0509618214045788E-9", "module": "C2", "scenario": "Energierückgewinnung"}, {"value": "2.5135102709692238E-9", "module": "C3", "scenario": "Energierückgewinnung"}, {"value": "0.0", "module": "C4", "scenario": "Energierückgewinnung"}, {"value": "-1.8138544046352632E-8", "module": "D", "scenario": "Energierückgewinnung"}, {"value": "0.0", "module": "C1", "scenario": "Recycling"}, {"value": "1.0509618214045788E-9", "module": "C2", "scenario": "Recycling"}, {"value": "-1.2515534651855717E-9", "module": "C3", "scenario": "Recycling"}, {"value": "0.0", "module": "C4", "scenario": "Recycling"}, {"value": "2.878514676811791E-8", "module": "D", "scenario": "Recycling"}, {"name": "referenceToUnitGroupDataSet", "value": {"shortDescription": [{"value": "CTUh", "lang": "en"}], "type": "unit group data set", "refObjectId": "d4c9523e-2d7e-49fd-8469-998f547d3a70", "version": "00.00.003", "uri": "../unitgroups/d4c9523e-2d7e-49fd-8469-998f547d3a70.xml"}}]}}, {"referenceToLCIAMethodDataSet": {"shortDescription": [{"value": "Potential Comparative Toxic Unit for humans - non-cancer effects (HTP-nc)", "lang": "en"}, {"value": "Potenzielle Toxizitätsvergleichseinheit für den Menschen - nicht kanzerogene Wirkung (HTP-nc)", "lang": "de"}], "type": "LCIA method data set", "refObjectId": "3af763a5-b7a1-48c9-9cee-1f223481fcef", "version": "01.00.003", "uri": "../lciamethods/3af763a5-b7a1-48c9-9cee-1f223481fcef.xml"}, "meanAmount": 0.0, "other": {"anies": [{"value": "7.477599153210919E-6", "module": "A1-A3"}, {"value": "1.8221200819926383E-7", "module": "A4"}, {"value": "1.031519321131761E-7", "module": "A5"}, {"value": "0.0", "module": "B1"}, {"value": "0.0", "module": "B2"}, {"value": "0.0", "module": "B3"}, {"value": "0.0", "module": "B4"}, {"value": "0.0", "module": "B5"}, {"value": "0.0", "module": "B6"}, {"value": "0.0", "module": "B7"}, {"value": "0.0", "module": "C1", "scenario": "Energierückgewinnung"}, {"value": "5.606523329208127E-8", "module": "C2", "scenario": "Energierückgewinnung"}, {"value": "8.966597138575686E-8", "module": "C3", "scenario": "Energierückgewinnung"}, {"value": "0.0", "module": "C4", "scenario": "Energierückgewinnung"}, {"value": "-7.168555267067367E-7", "module": "D", "scenario": "Energierückgewinnung"}, {"value": "0.0", "module": "C1", "scenario": "Recycling"}, {"value": "5.606523329208127E-8", "module": "C2", "scenario": "Recycling"}, {"value": "-4.6464176070801567E-8", "module": "C3", "scenario": "Recycling"}, {"value": "0.0", "module": "C4", "scenario": "Recycling"}, {"value": "4.0472872972182635E-5", "module": "D", "scenario": "Recycling"}, {"name": "referenceToUnitGroupDataSet", "value": {"shortDescription": [{"value": "CTUh", "lang": "en"}], "type": "unit group data set", "refObjectId": "d4c9523e-2d7e-49fd-8469-998f547d3a70", "version": "00.00.003", "uri": "../unitgroups/d4c9523e-2d7e-49fd-8469-998f547d3a70.xml"}}]}}, {"referenceToLCIAMethodDataSet": {"shortDescription": [{"value": "Potential Soil quality index (SQP)", "lang": "en"}, {"value": "Potenzieller Bodenqualitätsindex (SQP)", "lang": "de"}], "type": "LCIA method data set", "refObjectId": "b2ad6890-c78d-11e6-9d9d-cec0c932ce01", "version": "01.00.011", "uri": "../lciamethods/b2ad6890-c78d-11e6-9d9d-cec0c932ce01.xml"}, "meanAmount": 0.0, "other": {"anies": [{"value": "3854.4238901786644", "module": "A1-A3"}, {"value": "66.07051044660564", "module": "A4"}, {"value": "52.02279853195207", "module": "A5"}, {"value": "0.0", "module": "B1"}, {"value": "0.0", "module": "B2"}, {"value": "0.0", "module": "B3"}, {"value": "0.0", "module": "B4"}, {"value": "0.0", "module": "B5"}, {"value": "0.0", "module": "B6"}, {"value": "0.0", "module": "B7"}, {"value": "0.0", "module": "C1", "scenario": "Energierückgewinnung"}, {"value": "20.329387829725324", "module": "C2", "scenario": "Energierückgewinnung"}, {"value": "23.707731880516835", "module": "C3", "scenario": "Energierückgewinnung"}, {"value": "0.0", "module": "C4", "scenario": "Energierückgewinnung"}, {"value": "-291.81953680480103", "module": "D", "scenario": "Energierückgewinnung"}, {"value": "0.0", "module": "C1", "scenario": "Recycling"}, {"value": "20.329387829725324", "module": "C2", "scenario": "Recycling"}, {"value": "-462.8579718016301", "module": "C3", "scenario": "Recycling"}, {"value": "0.0", "module": "C4", "scenario": "Recycling"}, {"value": "-589.3706994162346", "module": "D", "scenario": "Recycling"}, {"name": "referenceToUnitGroupDataSet", "value": {"shortDescription": [{"value": "dimensionless", "lang": "en"}], "type": "unit group data set", "refObjectId": "f130951c-e67f-4f7f-8dd4-665de3974e18", "version": "00.00.004", "uri": "../unitgroups/f130951c-e67f-4f7f-8dd4-665de3974e18.xml"}}]}}]}, "otherAttributes": {"{http://www.indata.network/EPD/2019}epd-version": "1.2", "{http://www.okworx.com/ILCD/Extensions/2018/Profile}profile": "EN_15804_A2"}, "version": "1.1"}