{"processInformation": {"dataSetInformation": {"UUID": "328bb948-cbdc-4441-b232-64eea40b285d", "name": {"baseName": [{"value": "Enka®Grip&Drain", "lang": "en"}]}, "classificationInformation": {"classification": [{"class": [{"value": "Kunststoffe", "level": 0, "classId": "6"}, {"value": "Folien und Vliese", "level": 1, "classId": "6.6"}, {"value": "Technische Textilien", "level": 2, "classId": "6.6.07"}], "name": "OEKOBAU.DAT"}]}, "generalComment": [{"value": "The owner of this EPD shall be liable for the underlying information and evidence. The programme operator Kiwa-Ecobility Experts shall not be liable with respect to manufacturer data, life cycle assessment data and evidence. Note: The results table shown in this data set refers to the product Enka®Grip&Drain 7010/300.50PET/5004F/M110PP with the specific mass of 1.25 kg/m^2", "lang": "en"}], "other": {"anies": [{"scenario": [{"description": [{"value": "A scaling method was used to calculate the LCA results for the different Enka®Grip products. The scaling was done on the basis of mass per square meter. As a result of scaling there are results for both the fixed and the scalable part of the scaling function. The fixed part means that this number is the same for each product in the product group and the scalable part is the part that depends on the mass per unit area of the product. In order to calculate the correct number of each environmental impact category for each of the products in the product group, the following calculation should be done: [number fixed part]+([specific mass]*[number scalable part]). Note: The results table shown in this data set refers to the product Enka®Grip&Drain 7010/300.50PET/5004F/M110PP with the specific mass of 1.25 kg/m^2."}], "name": "Standard scenario", "default": true}]}]}}, "quantitativeReference": {"referenceToReferenceFlow": [1], "type": "Reference flow(s)"}, "time": {"referenceYear": 2022, "dataSetValidUntil": 2029, "timeRepresentativenessDescription": [{"value": "All process-specific data were collected for the operating year 2022.", "lang": "en"}], "other": {"anies": [{"name": "publicationDateOfEPD", "value": 1713225600000}]}}, "geography": {"locationOfOperationSupplyOrProduction": {"descriptionOfRestrictions": [{"value": "The input data are representative for Enka®Grip&Drain, a product of Freudenberg Performance Materials B.V.. The data are representative for European Union.\r", "lang": "en"}], "location": "EU-27"}}, "technology": {"technologyDescriptionAndIncludedProcesses": [{"value": "Enka®Grip&Drain is a multifunctional geocomposite consisting of 3 or 4 layers that combines veneer stabilization, reinforcement, drainage, filtration and seperation. The upper layer is a 10 mm thick 3D open structure mat which is made of polyamide mono-filaments that are firmly fused. The 3D mat features an open void up to 95 % allowing for soil retention capacity. The middle layer is a reinforcing PET woven geotextile providing tensile strength. The needed strength of the woven is calculated based on project specific needs. The third and down facing layer consists of a polypropylene V-shape structured drainage mat of 4 or 6 mm height that ensures optimal discharge of rain water when it saturates the cover soil. As an addition to this down facing layer there is the possibility to choose an additional polypropylene non-woven layer above or below the drainage core, providing further filtration and separation functionality. All layers are connected by means of stitching. The PET woven geotextile is wider than the structure mat, allowing for an overlap between lanes during installation. The rolls are 5 m wide, saving labor time on the job site. The Enka®Grip&Drain consists of a polyamide 3D Mat on top followed by a PET woven geotextile and PP V-shape drainage core on the bottom. Depending on project needs a PP needlepunched nonwoven can be added to one of both sides of the drainage core. The PET Wovens are produced in South-Korea and shipped by sea freight in containers. The polyamide 3D mat is produced at the Obernburg am Main site through a monofilament extrusion process. The polyamide chips are delivered by truck from Luxembourg. The PP V-shape drainage core is also made at the Obernburg am Main site via a similar extrusion process. The PP chips are delivered by truck from Germany. The PP needle punched non-wovens are shipped by truck from Hungary. At the Obernburg am Main site all components are sewn together on an assembly line to make the final product. The sewing yarns are delivered to the site per truck from Belgium. After sewing the product is wound up on 5m wide cardboard tubes and afterwards packaged with PE foil. The final good is a 5m wide roll with a standard length of 80m. When there are project specific needs the lengths and thus roll weight and diameter can vary depending on the required slope length.", "lang": "en"}], "technologicalApplicability": [{"value": "The multi-functional Enka®Grip&Drain is used as a combination of reinforced veneer stabilization and drainage on multi-layer lining systems, mostly in capping of waste containment and on geomembranes in retention ponds or reservoirs where it is installed on top of a geomembrane. Anchored in a trench on top of the slope, Enka®Grip&Drain delivers the required friction, tensile strength, anchorage resistance and drainage capacitie to stabilize the covering soil layer on large surfaces, preventing the soil from sliding. Because Enka®Grip&Drain includes a geosynthetic drainage layer, the product can replace or reduce the thickness of a traditional aggregate layer, thus minimizing transport movements to and from projects saving time, cost and emissions.", "lang": "en"}], "referenceToTechnologyFlowDiagrammOrPicture": [{"shortDescription": [{"value": "Flow chart Enka®Grip&Drain", "lang": "en"}], "type": "source data set", "refObjectId": "be1bd493-c92f-4208-8197-19901338f347", "version": "00.00.002"}]}}, "modellingAndValidation": {"LCIMethodAndAllocation": {"typeOfDataSet": "EPD", "other": {"anies": [{"name": "subType", "value": "specific dataset"}]}}, "dataSourcesTreatmentAndRepresentativeness": {"referenceToDataSource": [{"shortDescription": [{"value": "ecoinvent 3.6 database", "lang": "en"}], "type": "source data set", "refObjectId": "766b9973-5ee8-48a2-8098-72c8e20b369f", "version": "00.00.001"}, {"shortDescription": [{"value": "ecoinvent database (general)", "lang": "en"}], "type": "source data set", "refObjectId": "b497a91f-e14b-4b69-8f28-f50eb1576766", "version": "00.03.002"}], "useAdviceForDataSet": [{"value": "The results table shown in this data set refers to the product Enka®Grip&Drain 7010/300.50PET/5004F/M110PP with the specific mass of 1.25 kg/m^2.", "lang": "en"}], "other": {"anies": [{"name": "referenceToOriginalEPD", "value": {"shortDescription": {"value": "Enka®Grip&Drain EPD", "defaultValue": "Enka®Grip&Drain EPD", "lstrings": [{"lang": "en", "value": "Enka®Grip&Drain EPD"}]}, "version": {"version": 1, "majorVersion": 0, "minorVersion": 0, "subMinorVersion": 1, "zero": false, "versionString": "00.00.001"}, "type": "source data set", "uuid": {"uuid": "b13b46f7-4489-4e04-be1e-d43b9361eabc"}, "refObjectId": "b13b46f7-4489-4e04-be1e-d43b9361eabc", "versionAsString": "00.00.001", "resourceURLs": ["https://oekobaudat.de/OEKOBAU.DAT/resource/sources/b13b46f7-4489-4e04-be1e-d43b9361eabc/EPD-Kiwa-EE-170550-EN.pdf?version=00.00.001"]}}]}}, "validation": {"review": [{"reviewDetails": [{"value": "he independent verification is in accordance with the ISO 14025:2011.", "lang": "en"}], "referenceToNameOfReviewerAndInstitution": [{"shortDescription": [{"value": "Lucas Pedro Berman, Senda", "lang": "en"}], "type": "contact data set", "refObjectId": "2294137c-5a52-4a75-965f-770e74b24b10", "version": "00.00.002"}], "type": "Independent external review"}]}, "complianceDeclarations": {"compliance": [{"referenceToComplianceSystem": {"shortDescription": [{"value": "EN 15804+A2", "lang": "de"}, {"value": "EN 15804+A2", "lang": "en"}], "type": "source data set", "refObjectId": "c0016b33-8cf7-415c-ac6e-deba0d21440d", "version": "00.01.000"}}, {"referenceToComplianceSystem": {"shortDescription": [{"value": "ISO 14025", "lang": "en"}], "type": "source data set", "refObjectId": "4f2eb655-6e44-4874-a95a-e28f5442cd4d", "version": "00.00.001"}}]}}, "administrativeInformation": {"commissionerAndGoal": {"referenceToCommissioner": [{"shortDescription": [{"value": "Freudenberg Performance Materials B.V.", "lang": "en"}], "type": "contact data set", "refObjectId": "adc064d8-4c1f-4127-8ae9-cae8ea04141f", "version": "00.00.001"}]}, "dataGenerator": {"referenceToPersonOrEntityGeneratingTheDataSet": [{"shortDescription": [{"value": "Kiwa GmbH (Berlin)", "lang": "en"}], "type": "contact data set", "refObjectId": "3ea4a87a-3f88-4633-b7e7-1bbdd272be43", "version": "00.00.002"}]}, "dataEntryBy": {"timeStamp": 1726044218664, "referenceToDataSetFormat": [{"shortDescription": [{"value": "EPD Data Format Extensions v1.2", "lang": "en"}, {"value": "EPD-Datenformaterweiterungen v1.2", "lang": "de"}], "type": "source data set", "refObjectId": "a29449fd-aa2f-4de8-b5d7-4b06b43c6fde", "version": "00.01.000"}, {"shortDescription": [{"value": "ILCD format", "lang": "en"}], "type": "source data set", "refObjectId": "a97a0155-0234-4b87-b4ce-a45da52f2a40", "version": "01.00.001", "uri": "http://lca.jrc.ec.europa.eu/lcainfohub/sample_data/ilcd/sources/ILCD_Format_a97a0155-0234-4b87-b4ce-a45da52f2a40_01.00.000.xml"}], "referenceToPersonOrEntityEnteringTheData": {"shortDescription": [{"value": "Kiwa GmbH (Berlin)", "lang": "en"}], "type": "contact data set", "refObjectId": "3ea4a87a-3f88-4633-b7e7-1bbdd272be43", "version": "00.00.002"}}, "publicationAndOwnership": {"dataSetVersion": "00.00.011", "referenceToRegistrationAuthority": {"shortDescription": [{"value": "Kiwa-Ecobility Experts, Kiwa GmbH (Berlin)", "lang": "en"}], "type": "contact data set", "refObjectId": "eb52a9a8-9d0f-40ce-a5c9-7b78f5615e5a", "version": "00.00.002"}, "registrationNumber": "EPD-Kiwa-EE-170550-EN", "referenceToOwnershipOfDataSet": {"shortDescription": [{"value": "Freudenberg Performance Materials B.V.", "lang": "en"}], "type": "contact data set", "refObjectId": "adc064d8-4c1f-4127-8ae9-cae8ea04141f", "version": "00.00.001"}, "copyright": true, "licenseType": "Free of charge for all users and uses", "accessRestrictions": [{"value": "None.", "lang": "en"}], "other": {"anies": [{"name": "referenceToPublisher", "value": {"shortDescription": [{"value": "Kiwa-Ecobility Experts, Kiwa GmbH (Berlin)", "lang": "en"}], "type": "contact data set", "refObjectId": "eb52a9a8-9d0f-40ce-a5c9-7b78f5615e5a", "version": "00.00.002"}}]}}}, "exchanges": {"exchange": [{"dataSetInternalID": 1, "referenceToFlowDataSet": {"shortDescription": [{"value": "Enka®Grip&Drain", "lang": "en"}], "type": "flow data set", "refObjectId": "7ef77425-ec6e-4328-aa62-ba6cf9ebce8e", "version": "00.00.001"}, "meanAmount": 1.0, "resultingAmount": 1.0, "referenceFlow": true, "resolvedFlowVersion": "00.00.004", "resultingflowAmount": 1.0, "flowProperties": [{"name": [{"lang": "de", "value": "Fläche"}, {"lang": "en", "value": "Area"}], "uuid": "93a60a56-a3c8-19da-a746-0800200c9a66", "referenceFlowProperty": true, "meanValue": 1.0, "referenceUnit": "qm", "unitGroupUUID": "c20a03d7-bd90-4569-bc94-66cfd364dfc8"}], "materialProperties": [{"name": "layer thickness", "value": "0.016", "unit": "m", "unitDescription": "meters"}, {"name": "grammage", "value": "1.25", "unit": "kg/m^2", "unitDescription": "kilograms per square meter"}], "typeOfFlow": "Product flow", "classification": {"classHierarchy": "Kunststoffe / Folien und Vliese / Technische Textilien", "name": "OEKOBAU.DAT"}}, {"dataSetInternalID": 2, "referenceToFlowDataSet": {"shortDescription": [{"value": "Komponenten für die Wiederverwendung (CRU)", "lang": "de"}, {"value": "Components for re-use (CRU)", "lang": "en"}, {"value": "Componentes para su reutilización (CRU)", "lang": "es"}, {"value": "Komponenter för återanvändning (CRU)", "lang": "sv"}], "type": "flow data set", "refObjectId": "a2b32f97-3fc7-4af2-b209-525bc6426f33", "version": "30.00.002"}, "exchange direction": "OUTPUT", "meanAmount": 0.0, "other": {"anies": [{"value": "0.0", "module": "A1", "scenario": "Standard scenario"}, {"value": "0.0", "module": "A2", "scenario": "Standard scenario"}, {"value": "3.119352E-5", "module": "A3", "scenario": "Standard scenario"}, {"value": "0.0", "module": "C1", "scenario": "Standard scenario"}, {"value": "0.0", "module": "C2", "scenario": "Standard scenario"}, {"value": "0.0", "module": "C3", "scenario": "Standard scenario"}, {"value": "0.0", "module": "C4", "scenario": "Standard scenario"}, {"value": "0.0", "module": "D", "scenario": "Standard scenario"}, {"name": "referenceToUnitGroupDataSet", "value": {"shortDescription": [{"value": "kg"}], "type": "unit group data set", "refObjectId": "ad38d542-3fe9-439d-9b95-2f5f7752acaf", "uri": "../unitgroups/ad38d542-3fe9-439d-9b95-2f5f7752acaf"}}]}, "resolvedFlowVersion": "38.00.000", "flowProperties": [], "typeOfFlow": "Other flow", "classification": {"classHierarchy": "Quantities / Environmental quantities / EPD EN 15804 / LCI indicators", "name": "GaBiCategories"}}, {"dataSetInternalID": 3, "referenceToFlowDataSet": {"shortDescription": [{"value": "Exportierte elektrische Energie (EEE)", "lang": "de"}, {"value": "Exported electrical energy (EEE)", "lang": "en"}, {"value": "Energía exportada electrica (EEE)", "lang": "es"}, {"value": "Exporterad energi – elektrisk (EEE)", "lang": "sv"}], "type": "flow data set", "refObjectId": "4da0c987-2b76-40d6-9e9e-82a017aaaf29", "version": "30.00.002"}, "exchange direction": "OUTPUT", "meanAmount": 0.0, "other": {"anies": [{"value": "0.0", "module": "A1", "scenario": "Standard scenario"}, {"value": "0.0", "module": "A2", "scenario": "Standard scenario"}, {"value": "0.10931828488614", "module": "A3", "scenario": "Standard scenario"}, {"value": "0.0", "module": "C1", "scenario": "Standard scenario"}, {"value": "0.0", "module": "C2", "scenario": "Standard scenario"}, {"value": "0.0", "module": "C3", "scenario": "Standard scenario"}, {"value": "0.0", "module": "C4", "scenario": "Standard scenario"}, {"value": "7.54284726", "module": "D", "scenario": "Standard scenario"}, {"name": "referenceToUnitGroupDataSet", "value": {"shortDescription": [{"value": "MJ"}], "type": "unit group data set", "refObjectId": "93a60a57-a3c8-11da-a746-0800200c9a66", "uri": "../unitgroups/93a60a57-a3c8-11da-a746-0800200c9a66"}}]}, "resolvedFlowVersion": "38.00.000", "flowProperties": [], "typeOfFlow": "Other flow", "classification": {"classHierarchy": "Quantities / Environmental quantities / EPD EN 15804 / LCI indicators", "name": "GaBiCategories"}}, {"dataSetInternalID": 4, "referenceToFlowDataSet": {"shortDescription": [{"value": "Exportierte thermische Energie (EET)", "lang": "de"}, {"value": "Exported thermal energy (EET)", "lang": "en"}, {"value": "Energía exportada termal (EET)", "lang": "es"}, {"value": "Exporterad energi – termisk (EET)", "lang": "sv"}], "type": "flow data set", "refObjectId": "98daf38a-7a79-46d3-9a37-2b7bd0955810", "version": "30.00.002"}, "exchange direction": "OUTPUT", "meanAmount": 0.0, "other": {"anies": [{"value": "0.0", "module": "A1", "scenario": "Standard scenario"}, {"value": "0.0", "module": "A2", "scenario": "Standard scenario"}, {"value": "0.18827037952613002", "module": "A3", "scenario": "Standard scenario"}, {"value": "0.0", "module": "C1", "scenario": "Standard scenario"}, {"value": "0.0", "module": "C2", "scenario": "Standard scenario"}, {"value": "0.0", "module": "C3", "scenario": "Standard scenario"}, {"value": "0.0", "module": "C4", "scenario": "Standard scenario"}, {"value": "12.990459169999987", "module": "D", "scenario": "Standard scenario"}, {"name": "referenceToUnitGroupDataSet", "value": {"shortDescription": [{"value": "MJ"}], "type": "unit group data set", "refObjectId": "93a60a57-a3c8-11da-a746-0800200c9a66", "uri": "../unitgroups/93a60a57-a3c8-11da-a746-0800200c9a66"}}]}, "resolvedFlowVersion": "38.00.000", "flowProperties": [], "typeOfFlow": "Other flow", "classification": {"classHierarchy": "Quantities / Environmental quantities / EPD EN 15804 / LCI indicators", "name": "GaBiCategories"}}, {"dataSetInternalID": 5, "referenceToFlowDataSet": {"shortDescription": [{"value": "Gefährlicher Abfall zur Deponie (HWD)", "lang": "de"}, {"value": "Hazardous waste disposed (HWD)", "lang": "en"}, {"value": "Residuos peligrosos eliminados (HWD)", "lang": "es"}, {"value": "Farligt avfall (HWD)", "lang": "sv"}], "type": "flow data set", "refObjectId": "430f9e0f-59b2-46a0-8e0d-55e0e84948fc", "version": "30.00.002"}, "exchange direction": "OUTPUT", "meanAmount": 0.0, "other": {"anies": [{"value": "3.10052416585E-5", "module": "A1", "scenario": "Standard scenario"}, {"value": "5.286697771825E-6", "module": "A2", "scenario": "Standard scenario"}, {"value": "2.262874724975E-6", "module": "A3", "scenario": "Standard scenario"}, {"value": "1.228900316E-7", "module": "C1", "scenario": "Standard scenario"}, {"value": "1.359672384075E-6", "module": "C2", "scenario": "Standard scenario"}, {"value": "6.1384085E-6", "module": "C3", "scenario": "Standard scenario"}, {"value": "8.075415E-8", "module": "C4", "scenario": "Standard scenario"}, {"value": "-3.74260872436E-5", "module": "D", "scenario": "Standard scenario"}, {"name": "referenceToUnitGroupDataSet", "value": {"shortDescription": [{"value": "kg"}], "type": "unit group data set", "refObjectId": "ad38d542-3fe9-439d-9b95-2f5f7752acaf", "uri": "../unitgroups/ad38d542-3fe9-439d-9b95-2f5f7752acaf"}}]}, "resolvedFlowVersion": "38.00.000", "flowProperties": [], "typeOfFlow": "Other flow", "classification": {"classHierarchy": "Quantities / Environmental quantities / EPD EN 15804 / LCI indicators", "name": "GaBiCategories"}}, {"dataSetInternalID": 6, "referenceToFlowDataSet": {"shortDescription": [{"value": "Stoffe für die Energierückgewinnung (MER)", "lang": "de"}, {"value": "Materials for energy recovery (MER)", "lang": "en"}, {"value": "Materiales para valorización energética (recuperación de energía) (MER)", "lang": "es"}, {"value": "Material till energiåtervinning (MER)", "lang": "sv"}], "type": "flow data set", "refObjectId": "59a9181c-3aaf-46ee-8b13-2b3723b6e447", "version": "30.00.002"}, "exchange direction": "OUTPUT", "meanAmount": 0.0, "other": {"anies": [{"value": "0.0", "module": "A1", "scenario": "Standard scenario"}, {"value": "0.0", "module": "A2", "scenario": "Standard scenario"}, {"value": "0.0", "module": "A3", "scenario": "Standard scenario"}, {"value": "0.0", "module": "C1", "scenario": "Standard scenario"}, {"value": "0.0", "module": "C2", "scenario": "Standard scenario"}, {"value": "0.0", "module": "C3", "scenario": "Standard scenario"}, {"value": "0.0", "module": "C4", "scenario": "Standard scenario"}, {"value": "0.0", "module": "D", "scenario": "Standard scenario"}, {"name": "referenceToUnitGroupDataSet", "value": {"shortDescription": [{"value": "kg"}], "type": "unit group data set", "refObjectId": "ad38d542-3fe9-439d-9b95-2f5f7752acaf", "uri": "../unitgroups/ad38d542-3fe9-439d-9b95-2f5f7752acaf"}}]}, "resolvedFlowVersion": "38.00.000", "flowProperties": [], "typeOfFlow": "Other flow", "classification": {"classHierarchy": "Quantities / Environmental quantities / EPD EN 15804 / LCI indicators", "name": "GaBiCategories"}}, {"dataSetInternalID": 7, "referenceToFlowDataSet": {"shortDescription": [{"value": "Stoffe zum Recycling (MFR)", "lang": "de"}, {"value": "Materials for recycling (MFR)", "lang": "en"}, {"value": "Materiales para el reciclaje (MFR)", "lang": "es"}, {"value": "Material till återvinning (MFR)", "lang": "sv"}], "type": "flow data set", "refObjectId": "d7fe48a5-4103-49c8-9aae-b0b5dfdbd6ae", "version": "30.00.002"}, "exchange direction": "OUTPUT", "meanAmount": 0.0, "other": {"anies": [{"value": "0.0", "module": "A1", "scenario": "Standard scenario"}, {"value": "0.0", "module": "A2", "scenario": "Standard scenario"}, {"value": "0.00141971107", "module": "A3", "scenario": "Standard scenario"}, {"value": "0.0", "module": "C1", "scenario": "Standard scenario"}, {"value": "0.0", "module": "C2", "scenario": "Standard scenario"}, {"value": "0.0815", "module": "C3", "scenario": "Standard scenario"}, {"value": "0.0", "module": "C4", "scenario": "Standard scenario"}, {"value": "0.0", "module": "D", "scenario": "Standard scenario"}, {"name": "referenceToUnitGroupDataSet", "value": {"shortDescription": [{"value": "kg"}], "type": "unit group data set", "refObjectId": "ad38d542-3fe9-439d-9b95-2f5f7752acaf", "uri": "../unitgroups/ad38d542-3fe9-439d-9b95-2f5f7752acaf"}}]}, "resolvedFlowVersion": "38.00.000", "flowProperties": [], "typeOfFlow": "Other flow", "classification": {"classHierarchy": "Quantities / Environmental quantities / EPD EN 15804 / LCI indicators", "name": "GaBiCategories"}}, {"dataSetInternalID": 8, "referenceToFlowDataSet": {"shortDescription": [{"value": "Einsatz von Süßwasserressourcen (FW)", "lang": "de"}, {"value": "Use of net fresh water (FW)", "lang": "en"}, {"value": "Uso neto de recursos de agua dulce (FW)", "lang": "es"}, {"value": "Användning av sötvatten (FW)", "lang": "sv"}], "type": "flow data set", "refObjectId": "3cf952c8-f3a4-461d-8c96-96456ca62246", "version": "30.00.003"}, "exchange direction": "INPUT", "meanAmount": 0.0, "other": {"anies": [{"value": "0.0465225107589795", "module": "A1", "scenario": "Standard scenario"}, {"value": "2.848386856474E-4", "module": "A2", "scenario": "Standard scenario"}, {"value": "0.00230678837295555", "module": "A3", "scenario": "Standard scenario"}, {"value": "2.3228564365E-6", "module": "C1", "scenario": "Standard scenario"}, {"value": "6.535844197665E-5", "module": "C2", "scenario": "Standard scenario"}, {"value": "0.0062981681", "module": "C3", "scenario": "Standard scenario"}, {"value": "5.5546974999999993E-5", "module": "C4", "scenario": "Standard scenario"}, {"value": "-0.0030074778257337745", "module": "D", "scenario": "Standard scenario"}, {"name": "referenceToUnitGroupDataSet", "value": {"shortDescription": [{"value": "m3"}], "type": "unit group data set", "refObjectId": "cd950537-0a98-4044-9ba7-9f9a68d0a504", "uri": "../unitgroups/cd950537-0a98-4044-9ba7-9f9a68d0a504"}}]}, "resolvedFlowVersion": "38.00.000", "flowProperties": [], "typeOfFlow": "Other flow", "classification": {"classHierarchy": "Quantities / Environmental quantities / EPD EN 15804 / LCI indicators", "name": "GaBiCategories"}}, {"dataSetInternalID": 9, "referenceToFlowDataSet": {"shortDescription": [{"value": "Entsorgter nicht gefährlicher Abfall (NHWD)", "lang": "de"}, {"value": "Non hazardous waste dispose (NHWD)", "lang": "en"}, {"value": "Residuos no peligrosos eliminados (NHWD)", "lang": "es"}, {"value": "Icke-farligt avfall (NHWD)", "lang": "sv"}], "type": "flow data set", "refObjectId": "b29ef66b-e286-4afa-949f-62f1a7b4d7fa", "version": "30.00.002"}, "exchange direction": "OUTPUT", "meanAmount": 0.0, "other": {"anies": [{"value": "0.5689114761779931", "module": "A1", "scenario": "Standard scenario"}, {"value": "0.0550671322286389", "module": "A2", "scenario": "Standard scenario"}, {"value": "0.027080373634833475", "module": "A3", "scenario": "Standard scenario"}, {"value": "5.3419345853E-5", "module": "C1", "scenario": "Standard scenario"}, {"value": "0.03403531678991172", "module": "C2", "scenario": "Standard scenario"}, {"value": "0.0762916044", "module": "C3", "scenario": "Standard scenario"}, {"value": "0.21233717632500002", "module": "C4", "scenario": "Standard scenario"}, {"value": "-0.015203523266147274", "module": "D", "scenario": "Standard scenario"}, {"name": "referenceToUnitGroupDataSet", "value": {"shortDescription": [{"value": "kg"}], "type": "unit group data set", "refObjectId": "ad38d542-3fe9-439d-9b95-2f5f7752acaf", "uri": "../unitgroups/ad38d542-3fe9-439d-9b95-2f5f7752acaf"}}]}, "resolvedFlowVersion": "38.00.000", "flowProperties": [], "typeOfFlow": "Other flow", "classification": {"classHierarchy": "Quantities / Environmental quantities / EPD EN 15804 / LCI indicators", "name": "GaBiCategories"}}, {"dataSetInternalID": 10, "referenceToFlowDataSet": {"shortDescription": [{"value": "Nicht-erneuerbare Primärenergie als Energieträger (PENRE)", "lang": "de"}, {"value": "Use of non renewable primary energy (PENRE)", "lang": "en"}, {"value": "Uso de energía primaria no renovable, excluyendo los recursos de energía primaria no renovable utilizada como materia prima (PENRE)", "lang": "es"}, {"value": "Icke förnybar primärenergi - använd som energibärare (PENRE)", "lang": "sv"}], "type": "flow data set", "refObjectId": "ac857178-2b45-46ec-892a-a9a4332f0372", "version": "30.00.002"}, "exchange direction": "INPUT", "meanAmount": 0.0, "other": {"anies": [{"value": "48.992906386074104", "module": "A1", "scenario": "Standard scenario"}, {"value": "4.769429949829066", "module": "A2", "scenario": "Standard scenario"}, {"value": "2.250099246470443", "module": "A3", "scenario": "Standard scenario"}, {"value": "0.0479144135182203", "module": "C1", "scenario": "Standard scenario"}, {"value": "0.5696733485460577", "module": "C2", "scenario": "Standard scenario"}, {"value": "3.39286403614999", "module": "C3", "scenario": "Standard scenario"}, {"value": "0.056561667075", "module": "C4", "scenario": "Standard scenario"}, {"value": "-34.22299944403715", "module": "D", "scenario": "Standard scenario"}, {"name": "referenceToUnitGroupDataSet", "value": {"shortDescription": [{"value": "MJ"}], "type": "unit group data set", "refObjectId": "93a60a57-a3c8-11da-a746-0800200c9a66", "uri": "../unitgroups/93a60a57-a3c8-11da-a746-0800200c9a66"}}]}, "resolvedFlowVersion": "38.00.000", "flowProperties": [], "typeOfFlow": "Other flow", "classification": {"classHierarchy": "Quantities", "name": "GaBiCategories"}}, {"dataSetInternalID": 11, "referenceToFlowDataSet": {"shortDescription": [{"value": "Nicht-erneuerbare Primärenergie zur stofflichen Nutzung (PENRM)", "lang": "de"}, {"value": "Use of non renewable primary energy resources used as raw materials (PENRM)", "lang": "en"}, {"value": "Uso de la energía primaria no renovable utilizada como materia prima (PENRM)", "lang": "es"}, {"value": "Icke förnybar primärenergi - använd som råmaterial (PENRM)", "lang": "sv"}], "type": "flow data set", "refObjectId": "1421caa0-679d-4bf4-b282-0eb850ccae27", "version": "30.00.001"}, "exchange direction": "INPUT", "meanAmount": 0.0, "other": {"anies": [{"value": "49.952035249999774", "module": "A1", "scenario": "Standard scenario"}, {"value": "0.0", "module": "A2", "scenario": "Standard scenario"}, {"value": "1.45971244566305", "module": "A3", "scenario": "Standard scenario"}, {"value": "0.0", "module": "C1", "scenario": "Standard scenario"}, {"value": "0.0", "module": "C2", "scenario": "Standard scenario"}, {"value": "0.0", "module": "C3", "scenario": "Standard scenario"}, {"value": "0.0", "module": "C4", "scenario": "Standard scenario"}, {"value": "-2.3190743499999864", "module": "D", "scenario": "Standard scenario"}, {"name": "referenceToUnitGroupDataSet", "value": {"shortDescription": [{"value": "MJ"}], "type": "unit group data set", "refObjectId": "93a60a57-a3c8-11da-a746-0800200c9a66", "uri": "../unitgroups/93a60a57-a3c8-11da-a746-0800200c9a66"}}]}, "resolvedFlowVersion": "38.00.000", "flowProperties": [], "typeOfFlow": "Other flow", "classification": {"classHierarchy": "Quantities", "name": "GaBiCategories"}}, {"dataSetInternalID": 12, "referenceToFlowDataSet": {"shortDescription": [{"value": "Nicht erneuerbare Sekundärbrennstoffe (NRSF)", "lang": "de"}, {"value": "Use of non renewable secondary fuels (NRSF)", "lang": "en"}, {"value": "Uso de combustibles secundarios no renovables (NRSF)", "lang": "es"}, {"value": "Användning av ickeförnybara sekundära bränslen (NRSF)", "lang": "sv"}], "type": "flow data set", "refObjectId": "89def144-d39a-4287-b86f-efde453ddcb2", "version": "30.00.001"}, "exchange direction": "INPUT", "meanAmount": 0.0, "other": {"anies": [{"value": "0.0", "module": "A1", "scenario": "Standard scenario"}, {"value": "0.0", "module": "A2", "scenario": "Standard scenario"}, {"value": "0.0", "module": "A3", "scenario": "Standard scenario"}, {"value": "0.0", "module": "C1", "scenario": "Standard scenario"}, {"value": "0.0", "module": "C2", "scenario": "Standard scenario"}, {"value": "0.0", "module": "C3", "scenario": "Standard scenario"}, {"value": "0.0", "module": "C4", "scenario": "Standard scenario"}, {"value": "0.0", "module": "D", "scenario": "Standard scenario"}, {"name": "referenceToUnitGroupDataSet", "value": {"shortDescription": [{"value": "MJ"}], "type": "unit group data set", "refObjectId": "93a60a57-a3c8-11da-a746-0800200c9a66", "uri": "../unitgroups/93a60a57-a3c8-11da-a746-0800200c9a66"}}]}, "resolvedFlowVersion": "38.00.000", "flowProperties": [], "typeOfFlow": "Other flow", "classification": {"classHierarchy": "Quantities / Environmental quantities / EPD EN 15804 / LCI indicators", "name": "GaBiCategories"}}, {"dataSetInternalID": 13, "referenceToFlowDataSet": {"shortDescription": [{"value": "Entsorgter radioaktiver Abfall (RWD)", "lang": "de"}, {"value": "Radioactive waste disposed (RWD)", "lang": "en"}, {"value": "Residuos radiactivos eliminados (RWD)", "lang": "es"}, {"value": "Radioaktivt avfall (RWD) ", "lang": "sv"}], "type": "flow data set", "refObjectId": "3449546e-52ad-4b39-b809-9fb77cea8ff6", "version": "30.00.001"}, "exchange direction": "OUTPUT", "meanAmount": 0.0, "other": {"anies": [{"value": "1.499886034974E-4", "module": "A1", "scenario": "Standard scenario"}, {"value": "3.0962073342025E-5", "module": "A2", "scenario": "Standard scenario"}, {"value": "8.5138133462E-6", "module": "A3", "scenario": "Standard scenario"}, {"value": "3.132851896E-7", "module": "C1", "scenario": "Standard scenario"}, {"value": "3.523337863175E-6", "module": "C2", "scenario": "Standard scenario"}, {"value": "1.1460184749999999E-5", "module": "C3", "scenario": "Standard scenario"}, {"value": "3.1561925E-7", "module": "C4", "scenario": "Standard scenario"}, {"value": "-1.6258466185400002E-5", "module": "D", "scenario": "Standard scenario"}, {"name": "referenceToUnitGroupDataSet", "value": {"shortDescription": [{"value": "kg"}], "type": "unit group data set", "refObjectId": "ad38d542-3fe9-439d-9b95-2f5f7752acaf", "uri": "../unitgroups/ad38d542-3fe9-439d-9b95-2f5f7752acaf"}}]}, "resolvedFlowVersion": "38.00.000", "flowProperties": [], "typeOfFlow": "Other flow", "classification": {"classHierarchy": "Quantities / Environmental quantities / EPD EN 15804 / LCI indicators", "name": "GaBiCategories"}}, {"dataSetInternalID": 14, "referenceToFlowDataSet": {"shortDescription": [{"value": "Erneuerbare Primärenergie als Energieträger (PERE)", "lang": "de"}, {"value": "Use of renewable primary energy (PERE)", "lang": "en"}, {"value": "Uso de energía primaria renovable excluyendo los recursos de energía primaria renovable utilizada como materia prima (PERE)", "lang": "es"}, {"value": "Förnybar energi - använd som energibärare (PERE)", "lang": "sv"}], "type": "flow data set", "refObjectId": "20f32be5-0398-4288-9b6d-accddd195317", "version": "30.00.001"}, "exchange direction": "INPUT", "meanAmount": 0.0, "other": {"anies": [{"value": "3.9771334639222546", "module": "A1", "scenario": "Standard scenario"}, {"value": "0.0344857754137594", "module": "A2", "scenario": "Standard scenario"}, {"value": "0.7456558231316807", "module": "A3", "scenario": "Standard scenario"}, {"value": "2.440438130167E-4", "module": "C1", "scenario": "Standard scenario"}, {"value": "0.006717285251072275", "module": "C2", "scenario": "Standard scenario"}, {"value": "0.32896312", "module": "C3", "scenario": "Standard scenario"}, {"value": "9.4639505E-4", "module": "C4", "scenario": "Standard scenario"}, {"value": "-0.12686396856699086", "module": "D", "scenario": "Standard scenario"}, {"name": "referenceToUnitGroupDataSet", "value": {"shortDescription": [{"value": "MJ"}], "type": "unit group data set", "refObjectId": "93a60a57-a3c8-11da-a746-0800200c9a66", "uri": "../unitgroups/93a60a57-a3c8-11da-a746-0800200c9a66"}}]}, "resolvedFlowVersion": "38.00.000", "flowProperties": [], "typeOfFlow": "Other flow", "classification": {"classHierarchy": "Quantities", "name": "GaBiCategories"}}, {"dataSetInternalID": 15, "referenceToFlowDataSet": {"shortDescription": [{"value": "Erneuerbare Primärenergie zur stofflichen Nutzung (PERM)", "lang": "de"}, {"value": "Use of renewable primary energy resources used as raw materials (PERM)", "lang": "en"}, {"value": "Uso de energía primaria renovable utilizada como materia prima (PERM)", "lang": "es"}, {"value": "Förnybar energi - använd som råmaterial (PERM)", "lang": "sv"}], "type": "flow data set", "refObjectId": "fb3ec0de-548d-4508-aea5-00b73bf6f702", "version": "30.00.001"}, "exchange direction": "INPUT", "meanAmount": 0.0, "other": {"anies": [{"value": "0.0", "module": "A1", "scenario": "Standard scenario"}, {"value": "0.0", "module": "A2", "scenario": "Standard scenario"}, {"value": "0.65682736", "module": "A3", "scenario": "Standard scenario"}, {"value": "0.0", "module": "C1", "scenario": "Standard scenario"}, {"value": "0.0", "module": "C2", "scenario": "Standard scenario"}, {"value": "0.0", "module": "C3", "scenario": "Standard scenario"}, {"value": "0.0", "module": "C4", "scenario": "Standard scenario"}, {"value": "0.0", "module": "D", "scenario": "Standard scenario"}, {"name": "referenceToUnitGroupDataSet", "value": {"shortDescription": [{"value": "MJ"}], "type": "unit group data set", "refObjectId": "93a60a57-a3c8-11da-a746-0800200c9a66", "uri": "../unitgroups/93a60a57-a3c8-11da-a746-0800200c9a66"}}]}, "resolvedFlowVersion": "38.00.000", "flowProperties": [], "typeOfFlow": "Other flow", "classification": {"classHierarchy": "Quantities", "name": "GaBiCategories"}}, {"dataSetInternalID": 16, "referenceToFlowDataSet": {"shortDescription": [{"value": "Erneuerbare Sekundärbrennstoffe (RSF)", "lang": "de"}, {"value": "Use of renewable secondary fuels (RSF)", "lang": "en"}, {"value": "Uso de combustibles secundarios renovables (RSF)", "lang": "es"}, {"value": "Användning av förnybara sekundära bränslen (RSF)", "lang": "sv"}], "type": "flow data set", "refObjectId": "64333088-a55f-4aa2-9a31-c10b07816787", "version": "30.00.001"}, "exchange direction": "INPUT", "meanAmount": 0.0, "other": {"anies": [{"value": "0.0", "module": "A1", "scenario": "Standard scenario"}, {"value": "0.0", "module": "A2", "scenario": "Standard scenario"}, {"value": "0.0", "module": "A3", "scenario": "Standard scenario"}, {"value": "0.0", "module": "C1", "scenario": "Standard scenario"}, {"value": "0.0", "module": "C2", "scenario": "Standard scenario"}, {"value": "0.0", "module": "C3", "scenario": "Standard scenario"}, {"value": "0.0", "module": "C4", "scenario": "Standard scenario"}, {"value": "0.0", "module": "D", "scenario": "Standard scenario"}, {"name": "referenceToUnitGroupDataSet", "value": {"shortDescription": [{"value": "MJ"}], "type": "unit group data set", "refObjectId": "93a60a57-a3c8-11da-a746-0800200c9a66", "uri": "../unitgroups/93a60a57-a3c8-11da-a746-0800200c9a66"}}]}, "resolvedFlowVersion": "38.00.000", "flowProperties": [], "typeOfFlow": "Other flow", "classification": {"classHierarchy": "Quantities / Environmental quantities / EPD EN 15804 / LCI indicators", "name": "GaBiCategories"}}, {"dataSetInternalID": 17, "referenceToFlowDataSet": {"shortDescription": [{"value": "Einsatz von Sekundärstoffen (SM)", "lang": "de"}, {"value": "Use of secondary material (SM)", "lang": "en"}, {"value": "Uso de materiales secundarios (SM)", "lang": "es"}, {"value": "Användning av sekundära material (SM)", "lang": "sv"}], "type": "flow data set", "refObjectId": "c6a1f35f-2d09-4f54-8dfb-97e502e1ce92", "version": "30.00.001"}, "exchange direction": "INPUT", "meanAmount": 0.0, "other": {"anies": [{"value": "0.0", "module": "A1", "scenario": "Standard scenario"}, {"value": "0.0", "module": "A2", "scenario": "Standard scenario"}, {"value": "2.59946E-4", "module": "A3", "scenario": "Standard scenario"}, {"value": "0.0", "module": "C1", "scenario": "Standard scenario"}, {"value": "0.0", "module": "C2", "scenario": "Standard scenario"}, {"value": "0.0", "module": "C3", "scenario": "Standard scenario"}, {"value": "0.0", "module": "C4", "scenario": "Standard scenario"}, {"value": "0.0", "module": "D", "scenario": "Standard scenario"}, {"name": "referenceToUnitGroupDataSet", "value": {"shortDescription": [{"value": "kg"}], "type": "unit group data set", "refObjectId": "ad38d542-3fe9-439d-9b95-2f5f7752acaf", "uri": "../unitgroups/ad38d542-3fe9-439d-9b95-2f5f7752acaf"}}]}, "resolvedFlowVersion": "38.00.000", "flowProperties": [], "typeOfFlow": "Other flow", "classification": {"classHierarchy": "Quantities / Environmental quantities / EPD EN 15804 / LCI indicators", "name": "GaBiCategories"}}, {"dataSetInternalID": 18, "referenceToFlowDataSet": {"shortDescription": [{"value": "Total nicht erneuerbare Primärenergie (PENRT)", "lang": "de"}, {"value": "Total use of non renewable primary energy resource (PENRT)", "lang": "en"}, {"value": "Uso total de la energía primaria no renovable (energía primaria y recursos de energía primaria renovable utilizada como materia prima) (PENRT)", "lang": "es"}, {"value": "Icke förnybar primärenergi – total (PENRT)", "lang": "sv"}], "type": "flow data set", "refObjectId": "06159210-646b-4c8d-8583-da9b3b95a6c1", "version": "30.00.001"}, "exchange direction": "INPUT", "meanAmount": 0.0, "other": {"anies": [{"value": "98.94494140807397", "module": "A1", "scenario": "Standard scenario"}, {"value": "4.769429949829066", "module": "A2", "scenario": "Standard scenario"}, {"value": "3.7098116881334913", "module": "A3", "scenario": "Standard scenario"}, {"value": "0.0479144135182203", "module": "C1", "scenario": "Standard scenario"}, {"value": "0.5696733485460577", "module": "C2", "scenario": "Standard scenario"}, {"value": "3.39286403614999", "module": "C3", "scenario": "Standard scenario"}, {"value": "0.056561667075", "module": "C4", "scenario": "Standard scenario"}, {"value": "-36.54207379403715", "module": "D", "scenario": "Standard scenario"}, {"name": "referenceToUnitGroupDataSet", "value": {"shortDescription": [{"value": "MJ"}], "type": "unit group data set", "refObjectId": "93a60a57-a3c8-11da-a746-0800200c9a66", "uri": "../unitgroups/93a60a57-a3c8-11da-a746-0800200c9a66"}}]}, "resolvedFlowVersion": "38.00.000", "flowProperties": [], "typeOfFlow": "Other flow", "classification": {"classHierarchy": "Quantities / Environmental quantities / EPD EN 15804 / LCI indicators", "name": "GaBiCategories"}}, {"dataSetInternalID": 19, "referenceToFlowDataSet": {"shortDescription": [{"value": "Total erneuerbare Primärenergie (PERT)", "lang": "de"}, {"value": "Total use of renewable primary energy resources (PERT)", "lang": "en"}, {"value": "Uso total de la energía primaria renovable (energía primaria y recursos de energía primaria renovable utilizada como materia prima) (PERT)", "lang": "es"}, {"value": "Förnybar energi – total (PERT)", "lang": "sv"}], "type": "flow data set", "refObjectId": "53f97275-fa8a-4cdd-9024-65936002acd0", "version": "30.00.001"}, "exchange direction": "INPUT", "meanAmount": 0.0, "other": {"anies": [{"value": "3.9771334639222546", "module": "A1", "scenario": "Standard scenario"}, {"value": "0.0344857754137594", "module": "A2", "scenario": "Standard scenario"}, {"value": "1.4024831831316795", "module": "A3", "scenario": "Standard scenario"}, {"value": "2.440438130167E-4", "module": "C1", "scenario": "Standard scenario"}, {"value": "0.006717285251072275", "module": "C2", "scenario": "Standard scenario"}, {"value": "0.32896312", "module": "C3", "scenario": "Standard scenario"}, {"value": "9.4639505E-4", "module": "C4", "scenario": "Standard scenario"}, {"value": "-0.12686396856699086", "module": "D", "scenario": "Standard scenario"}, {"name": "referenceToUnitGroupDataSet", "value": {"shortDescription": [{"value": "MJ"}], "type": "unit group data set", "refObjectId": "93a60a57-a3c8-11da-a746-0800200c9a66", "uri": "../unitgroups/93a60a57-a3c8-11da-a746-0800200c9a66"}}]}, "resolvedFlowVersion": "38.00.000", "flowProperties": [], "typeOfFlow": "Other flow", "classification": {"classHierarchy": "Quantities / Environmental quantities / EPD EN 15804 / LCI indicators", "name": "GaBiCategories"}}]}, "LCIAResults": {"LCIAResult": [{"referenceToLCIAMethodDataSet": {"shortDescription": [{"value": "Potenzial für die Verknappung abiotischer Ressourcen – nicht fossile Ressourcen (ADPE)", "lang": "de"}, {"value": "Abiotic depletion potential - non-fossil resources (ADPE)", "lang": "en"}, {"value": "Abiotisk utarmningspotential icke fossila resurser (ADP-mm)", "lang": "sv"}], "type": "LCIA method data set", "refObjectId": "b2ad6494-c78d-11e6-9d9d-cec0c932ce01", "version": "01.00.013"}, "meanAmount": 0.0, "other": {"anies": [{"value": "4.0424668454700004E-5", "module": "A1", "scenario": "Standard scenario"}, {"value": "3.415991420975E-6", "module": "A2", "scenario": "Standard scenario"}, {"value": "1.588039799575E-6", "module": "A3", "scenario": "Standard scenario"}, {"value": "5.0275196E-9", "module": "C1", "scenario": "Standard scenario"}, {"value": "9.013842133750001E-7", "module": "C2", "scenario": "Standard scenario"}, {"value": "5.3036405E-6", "module": "C3", "scenario": "Standard scenario"}, {"value": "2.3985050000000002E-8", "module": "C4", "scenario": "Standard scenario"}, {"value": "-1.4411552963E-6", "module": "D", "scenario": "Standard scenario"}, {"name": "referenceToUnitGroupDataSet", "value": {"shortDescription": [{"value": "kg Sb-Äqv."}], "type": "unit group data set", "refObjectId": "54ccd2d9-a32a-4fc2-923d-f2c8c93e89d4", "uri": "../unitgroups/54ccd2d9-a32a-4fc2-923d-f2c8c93e89d4"}}]}}, {"referenceToLCIAMethodDataSet": {"shortDescription": [{"value": "Potenzial für die Verknappung abiotischer Ressourcen – fossile Brennstoffe (ADPF)", "lang": "de"}, {"value": "Abiotic depletion potential - fossil resources (ADPF)", "lang": "en"}, {"value": "Abiotisk utarmningspotential av fossila resurser (ADP-F)", "lang": "sv"}], "type": "LCIA method data set", "refObjectId": "b2ad6110-c78d-11e6-9d9d-cec0c932ce01", "version": "01.00.012"}, "meanAmount": 0.0, "other": {"anies": [{"value": "92.2651980438164", "module": "A1", "scenario": "Standard scenario"}, {"value": "4.492115115754492", "module": "A2", "scenario": "Standard scenario"}, {"value": "3.4808831791060615", "module": "A3", "scenario": "Standard scenario"}, {"value": "0.0451182743782754", "module": "C1", "scenario": "Standard scenario"}, {"value": "0.5365548610483309", "module": "C2", "scenario": "Standard scenario"}, {"value": "3.1925260363499905", "module": "C3", "scenario": "Standard scenario"}, {"value": "0.0532185668", "module": "C4", "scenario": "Standard scenario"}, {"value": "-33.06834591543035", "module": "D", "scenario": "Standard scenario"}, {"name": "referenceToUnitGroupDataSet", "value": {"shortDescription": [{"value": "MJ"}], "type": "unit group data set", "refObjectId": "93a60a57-a3c8-11da-a746-0800200c9a66", "uri": "../unitgroups/93a60a57-a3c8-11da-a746-0800200c9a66"}}]}}, {"referenceToLCIAMethodDataSet": {"shortDescription": [{"value": "Versauerungspotenzial, kumulierte Überschreitung (AP)", "lang": "de"}, {"value": "Acidification potential, Accumulated Exceedance (AP)", "lang": "en"}, {"value": "Försurningspotential på land och vatten (AP)", "lang": "sv"}], "type": "LCIA method data set", "refObjectId": "b5c611c6-def3-11e6-bf01-fe55135034f3", "version": "01.03.012", "uri": "http://lca.jrc.ec.europa.eu/lcainfohub/datasets/elcd/lciamethods/f6cbd466-253f-4145-a4bb-8dae7d266e89.xml"}, "meanAmount": 0.0, "other": {"anies": [{"value": "0.021145620752234102", "module": "A1", "scenario": "Standard scenario"}, {"value": "0.009854822160427601", "module": "A2", "scenario": "Standard scenario"}, {"value": "0.00102281255860115", "module": "A3", "scenario": "Standard scenario"}, {"value": "3.42873756248E-5", "module": "C1", "scenario": "Standard scenario"}, {"value": "2.0633064710990002E-4", "module": "C2", "scenario": "Standard scenario"}, {"value": "0.00188067645", "module": "C3", "scenario": "Standard scenario"}, {"value": "1.964752E-5", "module": "C4", "scenario": "Standard scenario"}, {"value": "-0.001822057786986425", "module": "D", "scenario": "Standard scenario"}, {"name": "referenceToUnitGroupDataSet", "value": {"shortDescription": [{"value": "mol H+ eqv."}], "type": "unit group data set", "refObjectId": "42e089ac-92bf-4bf2-8ca1-5fc40d18f2ed", "uri": "../unitgroups/42e089ac-92bf-4bf2-8ca1-5fc40d18f2ed"}}]}}, {"referenceToLCIAMethodDataSet": {"shortDescription": [{"value": "Eutrophierungspotenzial - Süßwasser (EP-freshwater)", "lang": "de"}, {"value": "Eutrophication potential - freshwater (EP-freshwater)", "lang": "en"}, {"value": "Övergödningspotential sötvatten (EP-fw)", "lang": "sv"}], "type": "LCIA method data set", "refObjectId": "b53ec18f-7377-4ad3-86eb-cc3f4f276b2b", "version": "01.00.012", "uri": "http://lca.jrc.ec.europa.eu/lcainfohub/datasets/elcd/lciamethods/a4630d5b-df2f-48ae-b3f2-5e5257606d68.xml"}, "meanAmount": 0.0, "other": {"anies": [{"value": "1.4451417947840002E-4", "module": "A1", "scenario": "Standard scenario"}, {"value": "1.694588724325E-6", "module": "A2", "scenario": "Standard scenario"}, {"value": "7.7355942227E-6", "module": "A3", "scenario": "Standard scenario"}, {"value": "1.19341971E-8", "module": "C1", "scenario": "Standard scenario"}, {"value": "3.5887636815E-7", "module": "C2", "scenario": "Standard scenario"}, {"value": "1.2600929249999998E-5", "module": "C3", "scenario": "Standard scenario"}, {"value": "4.044205E-8", "module": "C4", "scenario": "Standard scenario"}, {"value": "-3.73878913465E-6", "module": "D", "scenario": "Standard scenario"}, {"name": "referenceToUnitGroupDataSet", "value": {"shortDescription": [{"value": "kg P eqv."}], "type": "unit group data set", "refObjectId": "0429039d-a61d-4590-ba67-aa4a20a810a1", "uri": "../unitgroups/0429039d-a61d-4590-ba67-aa4a20a810a1"}}]}}, {"referenceToLCIAMethodDataSet": {"shortDescription": [{"value": "Eutrophierungspotenzial - Salzwasser (EP-marine)", "lang": "de"}, {"value": "Eutrophication potential - marine (EP-marine)", "lang": "en"}, {"value": "Övergödningspotential marin (EP-m)", "lang": "sv"}], "type": "LCIA method data set", "refObjectId": "b5c619fa-def3-11e6-bf01-fe55135034f3", "version": "02.00.012", "uri": "http://lca.jrc.ec.europa.eu/lcainfohub/datasets/elcd/lciamethods/5296e2be-060b-4e50-b033-d45f85f6ac92.xml"}, "meanAmount": 0.0, "other": {"anies": [{"value": "0.0044643430901737", "module": "A1", "scenario": "Standard scenario"}, {"value": "0.0024508387863486497", "module": "A2", "scenario": "Standard scenario"}, {"value": "2.2382893367837498E-4", "module": "A3", "scenario": "Standard scenario"}, {"value": "1.51363791995E-5", "module": "C1", "scenario": "Standard scenario"}, {"value": "7.2705972040425E-5", "module": "C2", "scenario": "Standard scenario"}, {"value": "5.146215E-4", "module": "C3", "scenario": "Standard scenario"}, {"value": "1.28338175E-5", "module": "C4", "scenario": "Standard scenario"}, {"value": "-4.966159099018E-4", "module": "D", "scenario": "Standard scenario"}, {"name": "referenceToUnitGroupDataSet", "value": {"shortDescription": [{"value": "kg N eqv."}], "type": "unit group data set", "refObjectId": "d05bb823-ecdf-4686-8c40-bf1d9257859f", "uri": "../unitgroups/d05bb823-ecdf-4686-8c40-bf1d9257859f"}}]}}, {"referenceToLCIAMethodDataSet": {"shortDescription": [{"value": "Eutrophierungspotenzial - Land (EP-terrestrial)", "lang": "de"}, {"value": "Eutrophication potential - terrestrial (EP-terrestrial)", "lang": "en"}, {"value": "Övergödningspotential total (EP-T)", "lang": "sv"}], "type": "LCIA method data set", "refObjectId": "b5c614d2-def3-11e6-bf01-fe55135034f3", "version": "01.02.011", "uri": "http://lca.jrc.ec.europa.eu/lcainfohub/datasets/elcd/lciamethods/40054970-5936-477c-9bec-29fa23b1cb77.xml"}, "meanAmount": 0.0, "other": {"anies": [{"value": "0.045635561473074196", "module": "A1", "scenario": "Standard scenario"}, {"value": "0.027241888961246304", "module": "A2", "scenario": "Standard scenario"}, {"value": "0.00243290388758875", "module": "A3", "scenario": "Standard scenario"}, {"value": "1.660810665023E-4", "module": "C1", "scenario": "Standard scenario"}, {"value": "8.015918329998251E-4", "module": "C2", "scenario": "Standard scenario"}, {"value": "0.00572797215", "module": "C3", "scenario": "Standard scenario"}, {"value": "7.211815E-5", "module": "C4", "scenario": "Standard scenario"}, {"value": "-0.005460151745354001", "module": "D", "scenario": "Standard scenario"}, {"name": "referenceToUnitGroupDataSet", "value": {"shortDescription": [{"value": "mol N eqv."}], "type": "unit group data set", "refObjectId": "71b4d617-0ec9-4d3f-b65e-e438940c2401", "uri": "../unitgroups/71b4d617-0ec9-4d3f-b65e-e438940c2401"}}]}}, {"referenceToLCIAMethodDataSet": {"shortDescription": [{"value": "Globales Erwärmungspotenzial - total (GWP-total)", "lang": "de"}, {"value": "Global Warming Potential - total (GWP-total)", "lang": "en"}, {"value": "Global uppvärmningspotential – Totalt (GWP-T)", "lang": "sv"}], "type": "LCIA method data set", "refObjectId": "6a37f984-a4b3-458a-a20a-64418c145fa2", "version": "04.00.018"}, "meanAmount": 0.0, "other": {"anies": [{"value": "5.68590453074851", "module": "A1", "scenario": "Standard scenario"}, {"value": "0.34287770368164905", "module": "A2", "scenario": "Standard scenario"}, {"value": "0.16933731589467343", "module": "A3", "scenario": "Standard scenario"}, {"value": "0.0032793335125099", "module": "C1", "scenario": "Standard scenario"}, {"value": "0.0356053251140439", "module": "C2", "scenario": "Standard scenario"}, {"value": "4.249389195199978", "module": "C3", "scenario": "Standard scenario"}, {"value": "0.030454491599999998", "module": "C4", "scenario": "Standard scenario"}, {"value": "-1.8576488802244082", "module": "D", "scenario": "Standard scenario"}, {"name": "referenceToUnitGroupDataSet", "value": {"shortDescription": [{"value": "kg CO2-Äqv."}], "type": "unit group data set", "refObjectId": "1ebf3012-d0db-4de2-aefd-ef30cedb0be1", "uri": "../unitgroups/1ebf3012-d0db-4de2-aefd-ef30cedb0be1"}}]}}, {"referenceToLCIAMethodDataSet": {"shortDescription": [{"value": "Globales Erwärmungspotenzial - fossil (GWP-fossil)", "lang": "de"}, {"value": "Global Warming Potential - fossil fuels (GWP-fossil)", "lang": "en"}, {"value": "Global uppvärmningspotential– fossil (GWP-f)", "lang": "sv"}], "type": "LCIA method data set", "refObjectId": "5f635281-343e-44fb-83df-1971b155e6b6", "version": "01.00.011"}, "meanAmount": 0.0, "other": {"anies": [{"value": "5.314942904552618", "module": "A1", "scenario": "Standard scenario"}, {"value": "0.3427232912770207", "module": "A2", "scenario": "Standard scenario"}, {"value": "0.23240716826117153", "module": "A3", "scenario": "Standard scenario"}, {"value": "0.0032781633982127", "module": "C1", "scenario": "Standard scenario"}, {"value": "0.035575865362707", "module": "C2", "scenario": "Standard scenario"}, {"value": "4.2483888606499995", "module": "C3", "scenario": "Standard scenario"}, {"value": "0.0304294632", "module": "C4", "scenario": "Standard scenario"}, {"value": "-1.8565392578672149", "module": "D", "scenario": "Standard scenario"}, {"name": "referenceToUnitGroupDataSet", "value": {"shortDescription": [{"value": "kg CO2-Äqv."}], "type": "unit group data set", "refObjectId": "1ebf3012-d0db-4de2-aefd-ef30cedb0be1", "uri": "../unitgroups/1ebf3012-d0db-4de2-aefd-ef30cedb0be1"}}]}}, {"referenceToLCIAMethodDataSet": {"shortDescription": [{"value": "Globales Erwärmungspotenzial - biogen (GWP-biogenic)", "lang": "de"}, {"value": "Global Warming Potential - biogenic (GWP-biogenic)", "lang": "en"}, {"value": "Global uppvärmningspotential – biogen (GWP-b)", "lang": "sv"}], "type": "LCIA method data set", "refObjectId": "2356e1ab-0185-4db5-86e5-16de51c7485c", "version": "01.00.007"}, "meanAmount": 0.0, "other": {"anies": [{"value": "0.367846146571085", "module": "A1", "scenario": "Standard scenario"}, {"value": "-6.676460002037502E-5", "module": "A2", "scenario": "Standard scenario"}, {"value": "-0.06380227118150832", "module": "A3", "scenario": "Standard scenario"}, {"value": "9.117507481E-7", "module": "C1", "scenario": "Standard scenario"}, {"value": "1.642355485975E-5", "module": "C2", "scenario": "Standard scenario"}, {"value": "6.625336E-4", "module": "C3", "scenario": "Standard scenario"}, {"value": "2.3806275E-5", "module": "C4", "scenario": "Standard scenario"}, {"value": "-0.0010265040630165", "module": "D", "scenario": "Standard scenario"}, {"name": "referenceToUnitGroupDataSet", "value": {"shortDescription": [{"value": "kg CO2-Äqv."}], "type": "unit group data set", "refObjectId": "1ebf3012-d0db-4de2-aefd-ef30cedb0be1", "uri": "../unitgroups/1ebf3012-d0db-4de2-aefd-ef30cedb0be1"}}]}}, {"referenceToLCIAMethodDataSet": {"shortDescription": [{"value": "Globales Erwärmungspotenzial - luluc (GWP-luluc)", "lang": "de"}, {"value": "Global Warming Potential - land use and land use change (GWP-luluc)", "lang": "en"}, {"value": "Global uppvärmningspotential - markanvändning och förändringar i markanvändning (GWP-luluc)", "lang": "sv"}], "type": "LCIA method data set", "refObjectId": "4331bbdb-978a-490d-8707-eeb047f01a55", "version": "01.00.007"}, "meanAmount": 0.0, "other": {"anies": [{"value": "0.0031154541971358", "module": "A1", "scenario": "Standard scenario"}, {"value": "2.211770046485E-4", "module": "A2", "scenario": "Standard scenario"}, {"value": "7.3242080186085E-4", "module": "A3", "scenario": "Standard scenario"}, {"value": "2.583635492E-7", "module": "C1", "scenario": "Standard scenario"}, {"value": "1.3036196477275E-5", "module": "C2", "scenario": "Standard scenario"}, {"value": "3.3805271E-4", "module": "C3", "scenario": "Standard scenario"}, {"value": "1.1172867499999999E-6", "module": "C4", "scenario": "Standard scenario"}, {"value": "-8.31182941752E-5", "module": "D", "scenario": "Standard scenario"}, {"name": "referenceToUnitGroupDataSet", "value": {"shortDescription": [{"value": "kg CO2-Äqv."}], "type": "unit group data set", "refObjectId": "1ebf3012-d0db-4de2-aefd-ef30cedb0be1", "uri": "../unitgroups/1ebf3012-d0db-4de2-aefd-ef30cedb0be1"}}]}}, {"referenceToLCIAMethodDataSet": {"shortDescription": [{"value": "Abbaupotenzial der stratosphärischen Ozonschicht (ODP)", "lang": "de"}, {"value": "Depletion potential of the stratospheric ozone layer (ODP)", "lang": "en"}, {"value": "Utarmningspotential för stratosfäriska ozonskiktet - ozonnedbrytning (ODP)", "lang": "sv"}], "type": "LCIA method data set", "refObjectId": "b5c629d6-def3-11e6-bf01-fe55135034f3", "version": "02.00.014", "uri": "http://lca.jrc.ec.europa.eu/lcainfohub/datasets/elcd/lciamethods/8b723200-3d8f-4eec-9e10-444edb029476.xml"}, "meanAmount": 0.0, "other": {"anies": [{"value": "2.0028566019999997E-7", "module": "A1", "scenario": "Standard scenario"}, {"value": "6.9751126975E-8", "module": "A2", "scenario": "Standard scenario"}, {"value": "1.14393559E-8", "module": "A3", "scenario": "Standard scenario"}, {"value": "7.07951E-10", "module": "C1", "scenario": "Standard scenario"}, {"value": "7.852447825E-9", "module": "C2", "scenario": "Standard scenario"}, {"value": "1.28824595E-7", "module": "C3", "scenario": "Standard scenario"}, {"value": "6.94786E-10", "module": "C4", "scenario": "Standard scenario"}, {"value": "-2.299571496E-7", "module": "D", "scenario": "Standard scenario"}, {"name": "referenceToUnitGroupDataSet", "value": {"shortDescription": [{"value": "kg CFC 11-Äquiv."}], "type": "unit group data set", "refObjectId": "d9e957c9-7309-4474-bf3a-7777df6c4e5b", "uri": "../unitgroups/d9e957c9-7309-4474-bf3a-7777df6c4e5b"}}]}}, {"referenceToLCIAMethodDataSet": {"shortDescription": [{"value": "Bildungspotenzial für troposphärisches Ozon (POCP)", "lang": "de"}, {"value": "Photochemical Ozone Creation Potential (POCP)", "lang": "en"}, {"value": "Potential till fotokemisk oxidantbildning – marknära ozon (POCP)", "lang": "sv"}], "type": "LCIA method data set", "refObjectId": "b5c610fe-def3-11e6-bf01-fe55135034f3", "version": "02.00.018", "uri": "http://lca.jrc.ec.europa.eu/lcainfohub/datasets/elcd/lciamethods/ec7836be-83eb-41da-bcda-1a6a3fe2d149.xml"}, "meanAmount": 0.0, "other": {"anies": [{"value": "0.0154643408955025", "module": "A1", "scenario": "Standard scenario"}, {"value": "0.0070859582139933255", "module": "A2", "scenario": "Standard scenario"}, {"value": "7.5212824317625E-4", "module": "A3", "scenario": "Standard scenario"}, {"value": "4.56640738959E-5", "module": "C1", "scenario": "Standard scenario"}, {"value": "2.2886024153290002E-4", "module": "C2", "scenario": "Standard scenario"}, {"value": "0.0015346485500000002", "module": "C3", "scenario": "Standard scenario"}, {"value": "2.734195E-5", "module": "C4", "scenario": "Standard scenario"}, {"value": "-0.001922632034298275", "module": "D", "scenario": "Standard scenario"}, {"name": "referenceToUnitGroupDataSet", "value": {"shortDescription": [{"value": "kg NMVOC eqv."}], "type": "unit group data set", "refObjectId": "d27c25f8-fbc1-44c6-b47b-4adbae4199c6", "uri": "../unitgroups/d27c25f8-fbc1-44c6-b47b-4adbae4199c6"}}]}}, {"referenceToLCIAMethodDataSet": {"shortDescription": [{"value": "Wasser-Entzugspotenzial (Benutzer) (WDP)", "lang": "de"}, {"value": "Water (user) deprivation potential (WDP)", "lang": "en"}, {"value": "Vattenfotavtryck (WDP)", "lang": "sv"}], "type": "LCIA method data set", "refObjectId": "b2ad66ce-c78d-11e6-9d9d-cec0c932ce01", "version": "03.00.016"}, "meanAmount": 0.0, "other": {"anies": [{"value": "1.86916772916324", "module": "A1", "scenario": "Standard scenario"}, {"value": "0.008106643599151975", "module": "A2", "scenario": "Standard scenario"}, {"value": "0.09055695198455865", "module": "A3", "scenario": "Standard scenario"}, {"value": "6.04595515868E-5", "module": "C1", "scenario": "Standard scenario"}, {"value": "0.001919629527629175", "module": "C2", "scenario": "Standard scenario"}, {"value": "0.214056943", "module": "C3", "scenario": "Standard scenario"}, {"value": "0.0022777046499999998", "module": "C4", "scenario": "Standard scenario"}, {"value": "-0.2148391075084296", "module": "D", "scenario": "Standard scenario"}, {"name": "referenceToUnitGroupDataSet", "value": {"shortDescription": [{"value": "m3 world eqv."}], "type": "unit group data set", "refObjectId": "6ae2df01-888e-46c8-b17d-49fa3869b476", "uri": "../unitgroups/6ae2df01-888e-46c8-b17d-49fa3869b476"}}]}}, {"referenceToLCIAMethodDataSet": {"shortDescription": [{"value": "Potenzielles Auftreten von Krankheiten aufgrund von Feinstaubemissionen (PM)", "lang": "de"}, {"value": "Potential incidence of disease due to PM emissions (PM)", "lang": "en"}, {"value": "Potential till utsläpp av partiklar (PM)", "lang": "sv"}], "type": "LCIA method data set", "refObjectId": "b5c602c6-def3-11e6-bf01-fe55135034f3", "version": "02.00.013", "uri": "http://lca.jrc.ec.europa.eu/lcainfohub/datasets/elcd/lciamethods/72ce3013-f678-4c6a-935b-f4752ff8901b.xml"}, "meanAmount": 0.0, "other": {"anies": [{"value": "1.8510137639999998E-7", "module": "A1", "scenario": "Standard scenario"}, {"value": "1.3405442874999998E-8", "module": "A2", "scenario": "Standard scenario"}, {"value": "8.819715374999999E-9", "module": "A3", "scenario": "Standard scenario"}, {"value": "9.088843E-10", "module": "C1", "scenario": "Standard scenario"}, {"value": "3.200532625E-9", "module": "C2", "scenario": "Standard scenario"}, {"value": "1.4926384500000003E-8", "module": "C3", "scenario": "Standard scenario"}, {"value": "3.690638E-10", "module": "C4", "scenario": "Standard scenario"}, {"value": "-7.3013556999999996E-9", "module": "D", "scenario": "Standard scenario"}, {"name": "referenceToUnitGroupDataSet", "value": {"shortDescription": [{"value": "disease incidence"}], "type": "unit group data set", "refObjectId": "3883559b-648f-4afc-8ba2-0bd24f3affa3", "uri": "../unitgroups/3883559b-648f-4afc-8ba2-0bd24f3affa3"}}]}}, {"referenceToLCIAMethodDataSet": {"shortDescription": [{"value": "Potenzielle Wirkung durch Exposition des Menschen mit U235 (IRP)", "lang": "de"}, {"value": "Potential Human exposure efficiency relative to U235 (IRP)", "lang": "en"}, {"value": "Exponeringseffektivitet relaterad till U235 (IR)", "lang": "sv"}], "type": "LCIA method data set", "refObjectId": "b5c632be-def3-11e6-bf01-fe55135034f3", "version": "01.00.013", "uri": "http://lca.jrc.ec.europa.eu/lcainfohub/datasets/elcd/lciamethods/a6f4cbc8-5388-44d6-9a67-53d05684f93e.xml"}, "meanAmount": 0.0, "other": {"anies": [{"value": "0.170605094548905", "module": "A1", "scenario": "Standard scenario"}, {"value": "0.019199421412379375", "module": "A2", "scenario": "Standard scenario"}, {"value": "0.0086275624397092", "module": "A3", "scenario": "Standard scenario"}, {"value": "1.933417855455E-4", "module": "C1", "scenario": "Standard scenario"}, {"value": "0.0022480864427399", "module": "C2", "scenario": "Standard scenario"}, {"value": "0.013193146000000001", "module": "C3", "scenario": "Standard scenario"}, {"value": "2.0820745E-4", "module": "C4", "scenario": "Standard scenario"}, {"value": "-0.0119705832634768", "module": "D", "scenario": "Standard scenario"}, {"name": "referenceToUnitGroupDataSet", "value": {"shortDescription": [{"value": "kBq U235 eqv."}], "type": "unit group data set", "refObjectId": "456b05bf-1415-44a9-9993-02452f554c09", "uri": "../unitgroups/456b05bf-1415-44a9-9993-02452f554c09"}}]}}, {"referenceToLCIAMethodDataSet": {"shortDescription": [{"value": "Potenzielle Toxizitätsvergleichseinheit für Ökosysteme (ETP-fw)", "lang": "de"}, {"value": "Potential Comparative Toxic Unit for ecosystems (ETP-fw)", "lang": "en"}, {"value": "Ecotoxicitet (ETP-fw) ", "lang": "sv"}], "type": "LCIA method data set", "refObjectId": "ee1082d1-b0f7-43ca-a1f0-21e2a4a74511", "version": "01.00.004", "uri": "http://lca.jrc.ec.europa.eu/lcainfohub/datasets/elcd/lciamethods/ee1082d1-b0f7-43ca-a1f0-21e2a4a74511.xml"}, "meanAmount": 0.0, "other": {"anies": [{"value": "56.53682235203082", "module": "A1", "scenario": "Standard scenario"}, {"value": "3.073556612556866", "module": "A2", "scenario": "Standard scenario"}, {"value": "3.9250299864943474", "module": "A3", "scenario": "Standard scenario"}, {"value": "0.0271982586007678", "module": "C1", "scenario": "Standard scenario"}, {"value": "0.47845730472981124", "module": "C2", "scenario": "Standard scenario"}, {"value": "53.18672480624977", "module": "C3", "scenario": "Standard scenario"}, {"value": "0.08972298655", "module": "C4", "scenario": "Standard scenario"}, {"value": "-2.3040717141446367", "module": "D", "scenario": "Standard scenario"}, {"name": "referenceToUnitGroupDataSet", "value": {"shortDescription": [{"value": "CTUe"}], "type": "unit group data set", "refObjectId": "aa959ded-f1eb-4efb-9c5c-2d60be36b3e6", "uri": "../unitgroups/aa959ded-f1eb-4efb-9c5c-2d60be36b3e6"}}]}}, {"referenceToLCIAMethodDataSet": {"shortDescription": [{"value": "Potenzielle Toxizitätsvergleichseinheit für den Menschen - kanzerogene Wirkung (HTP-c)", "lang": "de"}, {"value": "Potential Comparative Toxic Unit for humans - cancer effects (HTP-c)", "lang": "en"}, {"value": "Humantoxicitet – cancer (HTP-c)", "lang": "sv"}], "type": "LCIA method data set", "refObjectId": "2299222a-bbd8-474f-9d4f-4dd1f18aea7c", "version": "01.00.005", "uri": "http://lca.jrc.ec.europa.eu/lcainfohub/datasets/elcd/lciamethods/2299222a-bbd8-474f-9d4f-4dd1f18aea7c.xml"}, "meanAmount": 0.0, "other": {"anies": [{"value": "1.5667568E-9", "module": "A1", "scenario": "Standard scenario"}, {"value": "1.8781355000000002E-10", "module": "A2", "scenario": "Standard scenario"}, {"value": "1.0117937500000001E-10", "module": "A3", "scenario": "Standard scenario"}, {"value": "9.505E-13", "module": "C1", "scenario": "Standard scenario"}, {"value": "1.5518475E-11", "module": "C2", "scenario": "Standard scenario"}, {"value": "8.253813E-10", "module": "C3", "scenario": "Standard scenario"}, {"value": "1.4955E-12", "module": "C4", "scenario": "Standard scenario"}, {"value": "-1.38845875E-10", "module": "D", "scenario": "Standard scenario"}, {"name": "referenceToUnitGroupDataSet", "value": {"shortDescription": [{"value": "CTUh"}], "type": "unit group data set", "refObjectId": "d4c9523e-2d7e-49fd-8469-998f547d3a70", "uri": "../unitgroups/d4c9523e-2d7e-49fd-8469-998f547d3a70"}}]}}, {"referenceToLCIAMethodDataSet": {"shortDescription": [{"value": "Potenzielle Toxizitätsvergleichseinheit für den Menschen - nicht kanzerogene Wirkung (HTP-nc)", "lang": "de"}, {"value": "Potential Comparative Toxic Unit for humans - non-cancer effects (HTP-nc)", "lang": "en"}, {"value": "Humantoxicitet – icke cancer (HTP-nc)", "lang": "sv"}], "type": "LCIA method data set", "refObjectId": "3af763a5-b7a1-48c9-9cee-1f223481fcef", "version": "01.00.004", "uri": "http://lca.jrc.ec.europa.eu/lcainfohub/datasets/elcd/lciamethods/3af763a5-b7a1-48c9-9cee-1f223481fcef.xml"}, "meanAmount": 0.0, "other": {"anies": [{"value": "3.404983945E-8", "module": "A1", "scenario": "Standard scenario"}, {"value": "2.647774425E-9", "module": "A2", "scenario": "Standard scenario"}, {"value": "1.90197695E-9", "module": "A3", "scenario": "Standard scenario"}, {"value": "2.33565E-11", "module": "C1", "scenario": "Standard scenario"}, {"value": "5.233603249999999E-10", "module": "C2", "scenario": "Standard scenario"}, {"value": "1.68020875E-8", "module": "C3", "scenario": "Standard scenario"}, {"value": "4.26677E-11", "module": "C4", "scenario": "Standard scenario"}, {"value": "-2.2282071E-9", "module": "D", "scenario": "Standard scenario"}, {"name": "referenceToUnitGroupDataSet", "value": {"shortDescription": [{"value": "CTUh"}], "type": "unit group data set", "refObjectId": "d4c9523e-2d7e-49fd-8469-998f547d3a70", "uri": "../unitgroups/d4c9523e-2d7e-49fd-8469-998f547d3a70"}}]}}, {"referenceToLCIAMethodDataSet": {"shortDescription": [{"value": "Potenzieller Bodenqualitätsindex (SQP)", "lang": "de"}, {"value": "Potential Soil quality index (SQP)", "lang": "en"}, {"value": "Potentiell jordkvalitet index (SQP)", "lang": "sv"}], "type": "LCIA method data set", "refObjectId": "b2ad6890-c78d-11e6-9d9d-cec0c932ce01", "version": "01.00.014"}, "meanAmount": 0.0, "other": {"anies": [{"value": "12.407714999989931", "module": "A1", "scenario": "Standard scenario"}, {"value": "1.1411831879448935", "module": "A2", "scenario": "Standard scenario"}, {"value": "6.973991955776258", "module": "A3", "scenario": "Standard scenario"}, {"value": "0.0057581609652561", "module": "C1", "scenario": "Standard scenario"}, {"value": "0.465323082153423", "module": "C2", "scenario": "Standard scenario"}, {"value": "1.12631647215", "module": "C3", "scenario": "Standard scenario"}, {"value": "0.125684775075", "module": "C4", "scenario": "Standard scenario"}, {"value": "-0.5463517578310932", "module": "D", "scenario": "Standard scenario"}, {"name": "referenceToUnitGroupDataSet", "value": {"shortDescription": [{"value": "dimensionless"}], "type": "unit group data set", "refObjectId": "f130951c-e67f-4f7f-8dd4-665de3974e18", "uri": "../unitgroups/f130951c-e67f-4f7f-8dd4-665de3974e18"}}]}}]}, "otherAttributes": {"{http://www.okworx.com/ILCD/Extensions/2018/Profile}profile": "EN_15804_A2", "{http://www.indata.network/EPD/2019}epd-version": "1.2"}, "version": "1.1"}