{"processInformation": {"dataSetInformation": {"UUID": "35844c49-109e-4b6a-a529-86b6872ac9e8", "name": {"baseName": [{"value": "KOMBISAVE+ Universal Protection and Control Unit (NSE AG)", "lang": "en"}, {"value": "KOMBISAVE+ Universelle Schutz- und Steuereinheit (NSE AG)", "lang": "de"}]}, "classificationInformation": {"classification": [{"class": [{"value": "Gebäudetechnik", "level": 0, "classId": "8"}, {"value": "Elektro", "level": 1, "classId": "8.4"}, {"value": "Sicherungs- und Schaltschränke", "level": 2, "classId": "8.4.03"}], "name": "OEKOBAU.DAT"}, {"class": [{"value": "logistics, equipment, subcontractors, other", "level": 0, "classId": "28000000"}, {"value": "equipment, energy", "level": 1, "classId": "28050000"}], "name": "freeclass"}]}, "generalComment": [{"value": "The owner of this EPD shall be liable for the underlying information and evidence. The program operator Kiwa-Ecobility Experts shall not be liable with respect to manufacturer data, life cycle assessment data and evidence.\r\nThe EPD covers the cradle to grave of the product.\r\n", "lang": "en"}], "other": {"anies": [{"scenario": [{"description": [{"value": "Due to the large number of suppliers and associated data limitations, transport has been modelled using generic profiles representative of typical supply chains where specific data was not available. A company-specific transport profile has been applied to reflect realistic sourcing practices. The following assumptions apply. • For the end-of-life scenario, the EU scenarios have been selected, as the product market is in the EU. • Module A4 (Transport) is calculated based on the assumption that the product is transported over a distance of 424 km using the profile (ei3.9.1) Lorry (Truck), unspecified (default) | market group for (GLO). • Module A5: No losses are expected in the installation of product. • Among the B modules, only B6 (Operational energy) is considered relevant; all other B modules have been considered as not relevant due to a lack of significant impacts. • Repairs have been excluded, as they are very rarely necessary.", "lang": "en"}], "name": "Standard scenario", "default": true}]}, "<ns11:modules xmlns:ns11=\"http://openlca.org/epd_ilcd\" xmlns=\"http://lca.jrc.it/ILCD/Process\" xmlns:c=\"http://lca.jrc.it/ILCD/Contact\" xmlns:common=\"http://lca.jrc.it/ILCD/Common\" xmlns:epd=\"http://www.iai.kit.edu/EPD/2013\" xmlns:epd2=\"http://www.indata.network/EPD/2019\" xmlns:f=\"http://lca.jrc.it/ILCD/Flow\" xmlns:fp=\"http://lca.jrc.it/ILCD/FlowProperty\" xmlns:m=\"http://lca.jrc.it/ILCD/LCIAMethod\" xmlns:s=\"http://lca.jrc.it/ILCD/Source\" xmlns:u=\"http://lca.jrc.it/ILCD/UnitGroup\" name=\"A1\" scenario=\"Standard scenario\"/>", "<ns11:modules xmlns:ns11=\"http://openlca.org/epd_ilcd\" xmlns=\"http://lca.jrc.it/ILCD/Process\" xmlns:c=\"http://lca.jrc.it/ILCD/Contact\" xmlns:common=\"http://lca.jrc.it/ILCD/Common\" xmlns:epd=\"http://www.iai.kit.edu/EPD/2013\" xmlns:epd2=\"http://www.indata.network/EPD/2019\" xmlns:f=\"http://lca.jrc.it/ILCD/Flow\" xmlns:fp=\"http://lca.jrc.it/ILCD/FlowProperty\" xmlns:m=\"http://lca.jrc.it/ILCD/LCIAMethod\" xmlns:s=\"http://lca.jrc.it/ILCD/Source\" xmlns:u=\"http://lca.jrc.it/ILCD/UnitGroup\" name=\"A2\" scenario=\"Standard scenario\"/>", "<ns11:modules xmlns:ns11=\"http://openlca.org/epd_ilcd\" xmlns=\"http://lca.jrc.it/ILCD/Process\" xmlns:c=\"http://lca.jrc.it/ILCD/Contact\" xmlns:common=\"http://lca.jrc.it/ILCD/Common\" xmlns:epd=\"http://www.iai.kit.edu/EPD/2013\" xmlns:epd2=\"http://www.indata.network/EPD/2019\" xmlns:f=\"http://lca.jrc.it/ILCD/Flow\" xmlns:fp=\"http://lca.jrc.it/ILCD/FlowProperty\" xmlns:m=\"http://lca.jrc.it/ILCD/LCIAMethod\" xmlns:s=\"http://lca.jrc.it/ILCD/Source\" xmlns:u=\"http://lca.jrc.it/ILCD/UnitGroup\" name=\"A3\" scenario=\"Standard scenario\"/>", "<ns11:modules xmlns:ns11=\"http://openlca.org/epd_ilcd\" xmlns=\"http://lca.jrc.it/ILCD/Process\" xmlns:c=\"http://lca.jrc.it/ILCD/Contact\" xmlns:common=\"http://lca.jrc.it/ILCD/Common\" xmlns:epd=\"http://www.iai.kit.edu/EPD/2013\" xmlns:epd2=\"http://www.indata.network/EPD/2019\" xmlns:f=\"http://lca.jrc.it/ILCD/Flow\" xmlns:fp=\"http://lca.jrc.it/ILCD/FlowProperty\" xmlns:m=\"http://lca.jrc.it/ILCD/LCIAMethod\" xmlns:s=\"http://lca.jrc.it/ILCD/Source\" xmlns:u=\"http://lca.jrc.it/ILCD/UnitGroup\" name=\"A4\" scenario=\"Standard scenario\"/>", "<ns11:modules xmlns:ns11=\"http://openlca.org/epd_ilcd\" xmlns=\"http://lca.jrc.it/ILCD/Process\" xmlns:c=\"http://lca.jrc.it/ILCD/Contact\" xmlns:common=\"http://lca.jrc.it/ILCD/Common\" xmlns:epd=\"http://www.iai.kit.edu/EPD/2013\" xmlns:epd2=\"http://www.indata.network/EPD/2019\" xmlns:f=\"http://lca.jrc.it/ILCD/Flow\" xmlns:fp=\"http://lca.jrc.it/ILCD/FlowProperty\" xmlns:m=\"http://lca.jrc.it/ILCD/LCIAMethod\" xmlns:s=\"http://lca.jrc.it/ILCD/Source\" xmlns:u=\"http://lca.jrc.it/ILCD/UnitGroup\" name=\"A5\" scenario=\"Standard scenario\"/>", "<ns11:modules xmlns:ns11=\"http://openlca.org/epd_ilcd\" xmlns=\"http://lca.jrc.it/ILCD/Process\" xmlns:c=\"http://lca.jrc.it/ILCD/Contact\" xmlns:common=\"http://lca.jrc.it/ILCD/Common\" xmlns:epd=\"http://www.iai.kit.edu/EPD/2013\" xmlns:epd2=\"http://www.indata.network/EPD/2019\" xmlns:f=\"http://lca.jrc.it/ILCD/Flow\" xmlns:fp=\"http://lca.jrc.it/ILCD/FlowProperty\" xmlns:m=\"http://lca.jrc.it/ILCD/LCIAMethod\" xmlns:s=\"http://lca.jrc.it/ILCD/Source\" xmlns:u=\"http://lca.jrc.it/ILCD/UnitGroup\" name=\"B1\" scenario=\"Standard scenario\"/>", "<ns11:modules xmlns:ns11=\"http://openlca.org/epd_ilcd\" xmlns=\"http://lca.jrc.it/ILCD/Process\" xmlns:c=\"http://lca.jrc.it/ILCD/Contact\" xmlns:common=\"http://lca.jrc.it/ILCD/Common\" xmlns:epd=\"http://www.iai.kit.edu/EPD/2013\" xmlns:epd2=\"http://www.indata.network/EPD/2019\" xmlns:f=\"http://lca.jrc.it/ILCD/Flow\" xmlns:fp=\"http://lca.jrc.it/ILCD/FlowProperty\" xmlns:m=\"http://lca.jrc.it/ILCD/LCIAMethod\" xmlns:s=\"http://lca.jrc.it/ILCD/Source\" xmlns:u=\"http://lca.jrc.it/ILCD/UnitGroup\" name=\"B2\" scenario=\"Standard scenario\"/>", "<ns11:modules xmlns:ns11=\"http://openlca.org/epd_ilcd\" xmlns=\"http://lca.jrc.it/ILCD/Process\" xmlns:c=\"http://lca.jrc.it/ILCD/Contact\" xmlns:common=\"http://lca.jrc.it/ILCD/Common\" xmlns:epd=\"http://www.iai.kit.edu/EPD/2013\" xmlns:epd2=\"http://www.indata.network/EPD/2019\" xmlns:f=\"http://lca.jrc.it/ILCD/Flow\" xmlns:fp=\"http://lca.jrc.it/ILCD/FlowProperty\" xmlns:m=\"http://lca.jrc.it/ILCD/LCIAMethod\" xmlns:s=\"http://lca.jrc.it/ILCD/Source\" xmlns:u=\"http://lca.jrc.it/ILCD/UnitGroup\" name=\"B3\" scenario=\"Standard scenario\"/>", "<ns11:modules xmlns:ns11=\"http://openlca.org/epd_ilcd\" xmlns=\"http://lca.jrc.it/ILCD/Process\" xmlns:c=\"http://lca.jrc.it/ILCD/Contact\" xmlns:common=\"http://lca.jrc.it/ILCD/Common\" xmlns:epd=\"http://www.iai.kit.edu/EPD/2013\" xmlns:epd2=\"http://www.indata.network/EPD/2019\" xmlns:f=\"http://lca.jrc.it/ILCD/Flow\" xmlns:fp=\"http://lca.jrc.it/ILCD/FlowProperty\" xmlns:m=\"http://lca.jrc.it/ILCD/LCIAMethod\" xmlns:s=\"http://lca.jrc.it/ILCD/Source\" xmlns:u=\"http://lca.jrc.it/ILCD/UnitGroup\" name=\"B4\" scenario=\"Standard scenario\"/>", "<ns11:modules xmlns:ns11=\"http://openlca.org/epd_ilcd\" xmlns=\"http://lca.jrc.it/ILCD/Process\" xmlns:c=\"http://lca.jrc.it/ILCD/Contact\" xmlns:common=\"http://lca.jrc.it/ILCD/Common\" xmlns:epd=\"http://www.iai.kit.edu/EPD/2013\" xmlns:epd2=\"http://www.indata.network/EPD/2019\" xmlns:f=\"http://lca.jrc.it/ILCD/Flow\" xmlns:fp=\"http://lca.jrc.it/ILCD/FlowProperty\" xmlns:m=\"http://lca.jrc.it/ILCD/LCIAMethod\" xmlns:s=\"http://lca.jrc.it/ILCD/Source\" xmlns:u=\"http://lca.jrc.it/ILCD/UnitGroup\" name=\"B5\" scenario=\"Standard scenario\"/>", "<ns11:modules xmlns:ns11=\"http://openlca.org/epd_ilcd\" xmlns=\"http://lca.jrc.it/ILCD/Process\" xmlns:c=\"http://lca.jrc.it/ILCD/Contact\" xmlns:common=\"http://lca.jrc.it/ILCD/Common\" xmlns:epd=\"http://www.iai.kit.edu/EPD/2013\" xmlns:epd2=\"http://www.indata.network/EPD/2019\" xmlns:f=\"http://lca.jrc.it/ILCD/Flow\" xmlns:fp=\"http://lca.jrc.it/ILCD/FlowProperty\" xmlns:m=\"http://lca.jrc.it/ILCD/LCIAMethod\" xmlns:s=\"http://lca.jrc.it/ILCD/Source\" xmlns:u=\"http://lca.jrc.it/ILCD/UnitGroup\" name=\"B6\" scenario=\"Standard scenario\"/>", "<ns11:modules xmlns:ns11=\"http://openlca.org/epd_ilcd\" xmlns=\"http://lca.jrc.it/ILCD/Process\" xmlns:c=\"http://lca.jrc.it/ILCD/Contact\" xmlns:common=\"http://lca.jrc.it/ILCD/Common\" xmlns:epd=\"http://www.iai.kit.edu/EPD/2013\" xmlns:epd2=\"http://www.indata.network/EPD/2019\" xmlns:f=\"http://lca.jrc.it/ILCD/Flow\" xmlns:fp=\"http://lca.jrc.it/ILCD/FlowProperty\" xmlns:m=\"http://lca.jrc.it/ILCD/LCIAMethod\" xmlns:s=\"http://lca.jrc.it/ILCD/Source\" xmlns:u=\"http://lca.jrc.it/ILCD/UnitGroup\" name=\"B7\" scenario=\"Standard scenario\"/>", "<ns11:modules xmlns:ns11=\"http://openlca.org/epd_ilcd\" xmlns=\"http://lca.jrc.it/ILCD/Process\" xmlns:c=\"http://lca.jrc.it/ILCD/Contact\" xmlns:common=\"http://lca.jrc.it/ILCD/Common\" xmlns:epd=\"http://www.iai.kit.edu/EPD/2013\" xmlns:epd2=\"http://www.indata.network/EPD/2019\" xmlns:f=\"http://lca.jrc.it/ILCD/Flow\" xmlns:fp=\"http://lca.jrc.it/ILCD/FlowProperty\" xmlns:m=\"http://lca.jrc.it/ILCD/LCIAMethod\" xmlns:s=\"http://lca.jrc.it/ILCD/Source\" xmlns:u=\"http://lca.jrc.it/ILCD/UnitGroup\" name=\"C1\" scenario=\"Standard scenario\"/>", "<ns11:modules xmlns:ns11=\"http://openlca.org/epd_ilcd\" xmlns=\"http://lca.jrc.it/ILCD/Process\" xmlns:c=\"http://lca.jrc.it/ILCD/Contact\" xmlns:common=\"http://lca.jrc.it/ILCD/Common\" xmlns:epd=\"http://www.iai.kit.edu/EPD/2013\" xmlns:epd2=\"http://www.indata.network/EPD/2019\" xmlns:f=\"http://lca.jrc.it/ILCD/Flow\" xmlns:fp=\"http://lca.jrc.it/ILCD/FlowProperty\" xmlns:m=\"http://lca.jrc.it/ILCD/LCIAMethod\" xmlns:s=\"http://lca.jrc.it/ILCD/Source\" xmlns:u=\"http://lca.jrc.it/ILCD/UnitGroup\" name=\"C2\" scenario=\"Standard scenario\"/>", "<ns11:modules xmlns:ns11=\"http://openlca.org/epd_ilcd\" xmlns=\"http://lca.jrc.it/ILCD/Process\" xmlns:c=\"http://lca.jrc.it/ILCD/Contact\" xmlns:common=\"http://lca.jrc.it/ILCD/Common\" xmlns:epd=\"http://www.iai.kit.edu/EPD/2013\" xmlns:epd2=\"http://www.indata.network/EPD/2019\" xmlns:f=\"http://lca.jrc.it/ILCD/Flow\" xmlns:fp=\"http://lca.jrc.it/ILCD/FlowProperty\" xmlns:m=\"http://lca.jrc.it/ILCD/LCIAMethod\" xmlns:s=\"http://lca.jrc.it/ILCD/Source\" xmlns:u=\"http://lca.jrc.it/ILCD/UnitGroup\" name=\"C3\" scenario=\"Standard scenario\"/>", "<ns11:modules xmlns:ns11=\"http://openlca.org/epd_ilcd\" xmlns=\"http://lca.jrc.it/ILCD/Process\" xmlns:c=\"http://lca.jrc.it/ILCD/Contact\" xmlns:common=\"http://lca.jrc.it/ILCD/Common\" xmlns:epd=\"http://www.iai.kit.edu/EPD/2013\" xmlns:epd2=\"http://www.indata.network/EPD/2019\" xmlns:f=\"http://lca.jrc.it/ILCD/Flow\" xmlns:fp=\"http://lca.jrc.it/ILCD/FlowProperty\" xmlns:m=\"http://lca.jrc.it/ILCD/LCIAMethod\" xmlns:s=\"http://lca.jrc.it/ILCD/Source\" xmlns:u=\"http://lca.jrc.it/ILCD/UnitGroup\" name=\"C4\" scenario=\"Standard scenario\"/>", "<ns11:modules xmlns:ns11=\"http://openlca.org/epd_ilcd\" xmlns=\"http://lca.jrc.it/ILCD/Process\" xmlns:c=\"http://lca.jrc.it/ILCD/Contact\" xmlns:common=\"http://lca.jrc.it/ILCD/Common\" xmlns:epd=\"http://www.iai.kit.edu/EPD/2013\" xmlns:epd2=\"http://www.indata.network/EPD/2019\" xmlns:f=\"http://lca.jrc.it/ILCD/Flow\" xmlns:fp=\"http://lca.jrc.it/ILCD/FlowProperty\" xmlns:m=\"http://lca.jrc.it/ILCD/LCIAMethod\" xmlns:s=\"http://lca.jrc.it/ILCD/Source\" xmlns:u=\"http://lca.jrc.it/ILCD/UnitGroup\" name=\"D\" scenario=\"Standard scenario\"/>"]}}, "quantitativeReference": {"referenceToReferenceFlow": [1], "type": "Reference flow(s)"}, "time": {"referenceYear": 2024, "dataSetValidUntil": 2030, "timeRepresentativenessDescription": [{"value": "Primary data including all raw materials, packaging materials, energy consumption and ancillary materials was comprehensively collected for the reference year from 2024- 01-01 to 2024-12-31.", "lang": "en"}], "other": {"anies": [{"name": "publicationDateOfEPD", "value": 1755129600000}]}}, "geography": {"locationOfOperationSupplyOrProduction": {"descriptionOfRestrictions": [{"value": "The results of this EPD are representative for European Union, especially for DACH region.", "lang": "en"}], "location": "EU-27"}}, "technology": {"technologyDescriptionAndIncludedProcesses": [{"value": "This EPD is performed based on the representative product - KOMBISAVE+ RF (X2- I4U4X-B2C2-RS-EE), and covers the following product categories: - KOMBISAVE+ RN (overcurrent and motor protection), - KOMBISAVE+ RF (distance protection with ground fault detection), - KOMBISAVE+ RL (line differential and distance protection), - KOMBISAVE+ RQ (differential protection for two-winding transformers). The heaviest variant (KOMBISAVE+ RF X2-I4U5X-B4C2-RS-SO) is 0.217 kg (i.e. 4 %) heavier than the representative variant (5.473 kg, incl. packaging). But was less often sold in 2024 than the representative variant.\r\nThe product is manufactured using a variety of raw materials, including steel, PCBs, plastics and copper alloys. The PCB production takes place at external suppliers. All these components are then transported from suppliers to the assembly facility located in Wohlen. At the Wohlen factory, the final product is assembled through mechanical operations such as fixing, soldering and screwing. The assembled units are packaged using cardboard boxes for delivery to the installation site.\r\n", "lang": "en"}, {"value": "Diese EPD wurde auf Basis des repräsentativen Produkts KOMBISAVE+ RF (X2-I4U4X-B2C2-RS-EE) erstellt und umfasst folgende Produktkategorien: KOMBISAVE+ RN (Überstrom- und Motorschutz), KOMBISAVE+ RF (Distanzschutz mit Erdschlusserkennung), KOMBISAVE+ RL (Leitungsdifferential- und Distanzschutz), KOMBISAVE+ RQ (Differentialschutz für Zweischenkel-Transformatoren). Die schwerste Variante (KOMBISAVE+ RF X2-I4U5X-B4C2-RS-SO) ist 0,217 kg (d. h. 4 %) schwerer als die repräsentative Variante (5,473 kg inkl. Verpackung), wurde jedoch im Jahr 2024 seltener verkauft als die Referenzvariante.\r\nDas Produkt wird aus verschiedenen Rohmaterialien gefertigt, darunter Stahl, Leiterplatten (PCBs), Kunststoffe und Kupferlegierungen. Die Herstellung der Leiterplatten erfolgt bei externen Zulieferern. Alle diese Komponenten werden anschließend vom jeweiligen Lieferanten zum Montagewerk nach Wohlen transportiert. Im Werk Wohlen wird das Endprodukt durch mechanische Prozesse wie Befestigen, Löten und Verschrauben zusammengesetzt. Die montierten Einheiten werden für den Versand an den Installationsort in Kartonverpackungen verpackt.\r\n", "lang": "de"}], "technologicalApplicability": [{"value": "The main task of the KOMBISAVE+ is to protect the components of a power grid and its surroundings against power system faults. The available protection functions of the KOMBISAVE+ depend on the variant (RN, RF, RL or RQ) and include overcurrent protection, distance protection, ground fault protection, switch-on-to-fault protection, transformer differential protection, motor protection and line differential protection, among others. These protection functions can be activated and configured individually. The KOMBISAVE+ is delivered with a standard factory configuration. This standard configuration comprises the settings, the selection of protective functions, and the configuration of the optocoupler inputs, LEDs, relays outputs, etc. It is essential that the configuration is adapted to the specific use case. Input and output signals can be linked with protection and control functions via a comprehensive I/O-matrix. In the event of a fault in the protected object or in the protection unit, depending on the protection functions configured, an OFF command is generated, and a relay is activated if configured. The device is mainly deployed in Germany, Austria and Switzerland.", "lang": "en"}, {"value": "Die Hauptaufgabe des KOMBISAVE+ besteht darin, die Komponenten eines Stromnetzes sowie dessen Umgebung vor Fehlern im Energieversorgungssystem zu schützen. Die verfügbaren Schutzfunktionen des KOMBISAVE+ hängen von der jeweiligen Variante ab (RN, RF, RL oder RQ) und umfassen unter anderem Überstromschutz, Distanzschutz, Erdschlussschutz, Einschaltfehler-Schutz, Transformator-Differentialschutz, Motorschutz sowie Leitungsdifferentialschutz. Diese Schutzfunktionen können einzeln aktiviert und konfiguriert werden. Der KOMBISAVE+ wird mit einer standardmäßigen Werkskonfiguration ausgeliefert. Diese Standardkonfiguration beinhaltet die Einstellungen, die Auswahl der Schutzfunktionen sowie die Konfiguration der Optokoppler-Eingänge, LEDs, Relaisausgänge usw. Es ist unerlässlich, dass die Konfiguration an den jeweiligen Anwendungsfall angepasst wird. Eingangs- und Ausgangssignale können über eine umfassende I/O-Matrix mit Schutz- und Steuerfunktionen verknüpft werden. Im Falle eines Fehlers am geschützten Objekt oder in der Schutzeinheit wird, abhängig von den konfigurierten Schutzfunktionen, ein AUS-Befehl generiert und, falls konfiguriert, ein Relais aktiviert. Das Gerät wird hauptsächlich in Deutschland, Österreich und der Schweiz eingesetzt.", "lang": "de"}]}}, "modellingAndValidation": {"LCIMethodAndAllocation": {"typeOfDataSet": "EPD", "referenceToLCAMethodDetails": [{"shortDescription": [{"value": "General Programme Instructions “Product Level”, Kiwa-Ecobility Experts", "lang": "en"}], "type": "source data set", "refObjectId": "7140e28f-f6b8-49ff-a325-02fe509586fa", "version": "00.00.001"}, {"shortDescription": [{"value": "Kiwa-EE GPI R.3.0 Annex B1 (2025)", "lang": "en"}], "type": "source data set", "refObjectId": "ae3f940b-093c-4805-9791-2af06cd6577f", "version": "00.00.001"}, {"shortDescription": [{"value": "EN 50693:2019 Product category rules for life cycle assessments of electronic and electrical products and systems", "lang": "en"}], "type": "source data set", "refObjectId": "457d17d7-100d-4eaa-8757-9b5c7eb0d4a5", "version": "00.00.002"}, {"shortDescription": [{"value": "EPDItaly007 Core PCR EN 50693 - ELECTRONIC AND ELECTRICAL PRODUCTS AND SYSTEMS, REV. 3", "lang": "en"}], "type": "source data set", "refObjectId": "9e5050d6-c47f-4c71-9d42-539b71cf6ae7", "version": "00.00.001"}], "other": {"anies": [{"name": "subType", "value": "specific dataset"}]}}, "dataSourcesTreatmentAndRepresentativeness": {"referenceToDataSource": [{"shortDescription": [{"value": "ecoinvent 3.9.1 database", "lang": "en"}], "type": "source data set", "refObjectId": "e2034c8f-9d74-46f2-8fce-1f0c5c5cebeb", "version": "00.00.001"}, {"shortDescription": [{"value": "ecoinvent database (general)", "lang": "en"}], "type": "source data set", "refObjectId": "b497a91f-e14b-4b69-8f28-f50eb1576766", "version": "00.03.002"}], "useAdviceForDataSet": [{"value": "The main task of the KOMBISAVE+ is to protect the components of a power grid and its surroundings against power system faults. The available protection functions of the KOMBISAVE+ depend on the variant (RN, RF, RL or RQ) and include overcurrent protection, distance protection, ground fault protection, switch-on-to-fault protection, transformer differential protection, motor protection and line differential protection, among others. These protection functions can be activated and configured individually. The KOMBISAVE+ is delivered with a standard factory configuration. This standard configuration comprises the settings, the selection of protective functions, and the configuration of the optocoupler inputs, LEDs, relays outputs, etc. It is essential that the configuration is adapted to the specific use case. Input and output signals can be linked with protection and control functions via a comprehensive I/O-matrix. In the event of a fault in the protected object or in the protection unit, depending on the protection functions configured, an OFF command is generated, and a relay is activated if configured. The device is mainly deployed in Germany, Austria and Switzerland.", "lang": "en"}], "other": {"anies": [{"name": "referenceToOriginalEPD", "value": {"shortDescription": {"value": "KOMBISAVE+ Universal Protection and Control Unit EPD", "defaultValue": "KOMBISAVE+ Universal Protection and Control Unit EPD", "lstrings": [{"lang": "en", "value": "KOMBISAVE+ Universal Protection and Control Unit EPD"}]}, "version": {"version": 1, "majorVersion": 0, "minorVersion": 0, "subMinorVersion": 1, "zero": false, "versionString": "00.00.001"}, "type": "source data set", "uuid": {"uuid": "33524b36-50fb-4941-9baa-7ac66779536d"}, "refObjectId": "33524b36-50fb-4941-9baa-7ac66779536d", "versionAsString": "00.00.001", "resourceURLs": ["https://oekobaudat.de/OEKOBAU.DAT/resource/sources/33524b36-50fb-4941-9baa-7ac66779536d/EPD-Kiwa-EE-000448-EN.pdf?version=00.00.001"]}}]}}, "validation": {"review": [{"reviewDetails": [{"value": "The independent verification is in accordance with the ISO 14025:2011.", "lang": "en"}], "referenceToNameOfReviewerAndInstitution": [{"shortDescription": [{"value": "Patrick Wortner, PeoplePlanetProfit GmbH & Co. KG.", "lang": "en"}], "type": "contact data set", "refObjectId": "8a83a8a2-e1da-4c93-b2f4-1d31fce7b233", "version": "00.00.001"}], "type": "Independent external review"}]}, "complianceDeclarations": {"compliance": [{"referenceToComplianceSystem": {"shortDescription": [{"value": "ISO 14025", "lang": "en"}], "type": "source data set", "refObjectId": "4f2eb655-6e44-4874-a95a-e28f5442cd4d", "version": "00.00.001"}}, {"referenceToComplianceSystem": {"shortDescription": [{"value": "EN 15804+A2 (EF 3.1)", "lang": "de"}, {"value": "EN 15804+A2 (EF 3.1)", "lang": "en"}], "type": "source data set", "refObjectId": "d4aa3ec7-b1d7-4a4a-a6cb-37af88dcc902", "version": "00.01.000"}}]}}, "administrativeInformation": {"commissionerAndGoal": {"referenceToCommissioner": [{"shortDescription": [{"value": "NSE AG", "lang": "en"}], "type": "contact data set", "refObjectId": "de5ad438-1ef2-40f4-9166-cbf43998510a", "version": "00.00.001"}]}, "dataGenerator": {"referenceToPersonOrEntityGeneratingTheDataSet": [{"shortDescription": [{"value": "Kiwa GmbH (Berlin)", "lang": "en"}], "type": "contact data set", "refObjectId": "3ea4a87a-3f88-4633-b7e7-1bbdd272be43", "version": "00.00.002"}]}, "dataEntryBy": {"timeStamp": 1759399988878, "referenceToDataSetFormat": [{"shortDescription": [{"value": "EPD Data Format Extensions v1.2", "lang": "en"}, {"value": "EPD-Datenformaterweiterungen v1.2", "lang": "de"}], "type": "source data set", "refObjectId": "a29449fd-aa2f-4de8-b5d7-4b06b43c6fde", "version": "00.01.000"}, {"shortDescription": [{"value": "ILCD format", "lang": "en"}], "type": "source data set", "refObjectId": "a97a0155-0234-4b87-b4ce-a45da52f2a40", "version": "01.00.000", "uri": "http://lca.jrc.ec.europa.eu/lcainfohub/sample_data/ilcd/sources/ILCD_Format_a97a0155-0234-4b87-b4ce-a45da52f2a40_01.00.000.xml"}], "referenceToPersonOrEntityEnteringTheData": {"shortDescription": [{"value": "Kiwa-Ecobility Experts, Kiwa GmbH (Berlin)", "lang": "en"}], "type": "contact data set", "refObjectId": "eb52a9a8-9d0f-40ce-a5c9-7b78f5615e5a", "version": "00.00.002"}}, "publicationAndOwnership": {"dataSetVersion": "00.00.003", "referenceToRegistrationAuthority": {"shortDescription": [{"value": "Kiwa-Ecobility Experts, Kiwa GmbH (Berlin)", "lang": "en"}], "type": "contact data set", "refObjectId": "eb52a9a8-9d0f-40ce-a5c9-7b78f5615e5a", "version": "00.00.002"}, "registrationNumber": "EPD-Kiwa-EE-000448-EN", "referenceToOwnershipOfDataSet": {"shortDescription": [{"value": "NSE AG", "lang": "en"}], "type": "contact data set", "refObjectId": "de5ad438-1ef2-40f4-9166-cbf43998510a", "version": "00.00.001"}, "copyright": true, "licenseType": "Free of charge for all users and uses", "accessRestrictions": [{"value": "None.", "lang": "en"}], "other": {"anies": [{"name": "referenceToPublisher", "value": {"shortDescription": [{"value": "Kiwa-Ecobility Experts, Kiwa GmbH (Berlin)", "lang": "en"}], "type": "contact data set", "refObjectId": "eb52a9a8-9d0f-40ce-a5c9-7b78f5615e5a", "version": "00.00.002"}}]}}}, "exchanges": {"exchange": [{"dataSetInternalID": 1, "referenceToFlowDataSet": {"shortDescription": [{"value": "KOMBISAVE+ Universal Protection and Control Unit", "lang": "en"}], "type": "flow data set", "refObjectId": "9f53fc6a-f213-4d07-ba8e-b1c85f6b4541", "version": "00.00.001"}, "meanAmount": 1.0, "resultingAmount": 1.0, "referenceFlow": true, "resultingflowAmount": 1.0, "flowProperties": [{"name": [{"lang": "en", "value": "Carbon content (biogenic)"}], "uuid": "62e503ce-544a-4599-b2ad-bcea15a7bf20", "meanValue": 0.0}, {"name": [{"lang": "de", "value": "Anzahl"}, {"lang": "en", "value": "Number of pieces"}], "uuid": "01846770-4cfe-4a25-8ad9-919d8d378345", "referenceFlowProperty": true, "meanValue": 1.0, "referenceUnit": "pcs.", "unitGroupUUID": "934110e3-baf4-49e9-992c-3d8109a6aafb"}, {"name": [{"lang": "en", "value": "Carbon content (biogenic) - packaging"}], "uuid": "262a541b-209e-44cc-a426-33bce30de7b1", "meanValue": 0.3287}], "materialProperties": [{"name": "weight per piece", "value": "4.723", "unit": "kg"}], "typeOfFlow": "Product flow", "classification": {"classHierarchy": "Gebäudetechnik / Elektro / Sicherungs- und Schaltschränke", "name": "OEKOBAU.DAT"}}, {"dataSetInternalID": 2, "referenceToFlowDataSet": {"shortDescription": [{"value": "Components for re-use (CRU)", "lang": "en"}, {"value": "Komponenten für die Wiederverwendung (CRU)", "lang": "de"}, {"value": "Componentes para su reutilización (CRU)", "lang": "es"}], "type": "flow data set", "refObjectId": "a2b32f97-3fc7-4af2-b209-525bc6426f33", "version": "30.00.000", "uri": "../flows/a2b32f97-3fc7-4af2-b209-525bc6426f33.xml"}, "exchange direction": "OUTPUT", "meanAmount": 0.0, "other": {"anies": [{"value": "0.0", "module": "A1", "scenario": "Standard scenario"}, {"value": "0.0", "module": "A2", "scenario": "Standard scenario"}, {"value": "0.0", "module": "A3", "scenario": "Standard scenario"}, {"value": "0.0", "module": "A4", "scenario": "Standard scenario"}, {"value": "0.0", "module": "A5", "scenario": "Standard scenario"}, {"value": "0.0", "module": "B1", "scenario": "Standard scenario"}, {"value": "0.0", "module": "B2", "scenario": "Standard scenario"}, {"value": "0.0", "module": "B3", "scenario": "Standard scenario"}, {"value": "0.0", "module": "B4", "scenario": "Standard scenario"}, {"value": "0.0", "module": "B5", "scenario": "Standard scenario"}, {"value": "0.0", "module": "B6", "scenario": "Standard scenario"}, {"value": "0.0", "module": "B7", "scenario": "Standard scenario"}, {"value": "0.0", "module": "C1", "scenario": "Standard scenario"}, {"value": "0.0", "module": "C2", "scenario": "Standard scenario"}, {"value": "0.0", "module": "C3", "scenario": "Standard scenario"}, {"value": "0.0", "module": "C4", "scenario": "Standard scenario"}, {"value": "0.0", "module": "D", "scenario": "Standard scenario"}, {"name": "referenceToUnitGroupDataSet", "value": {"shortDescription": [{"value": "kg", "lang": "en"}], "type": "unit group data set", "refObjectId": "ad38d542-3fe9-439d-9b95-2f5f7752acaf", "version": "30.00.000", "uri": "../unitgroups/ad38d542-3fe9-439d-9b95-2f5f7752acaf.xml"}}]}, "flowProperties": [], "typeOfFlow": "Other flow", "classification": {"classHierarchy": "Größen / Umweltliche Größen / EPD EN 15804 / LCI Indikatoren", "name": "GaBiCategories"}}, {"dataSetInternalID": 3, "referenceToFlowDataSet": {"shortDescription": [{"value": "Exported electrical energy (EEE)", "lang": "en"}, {"value": "Exportierte elektrische Energie (EEE)", "lang": "de"}, {"value": "Energía exportada electrica (EEE)", "lang": "es"}], "type": "flow data set", "refObjectId": "4da0c987-2b76-40d6-9e9e-82a017aaaf29", "version": "30.00.000", "uri": "../flows/4da0c987-2b76-40d6-9e9e-82a017aaaf29.xml"}, "exchange direction": "OUTPUT", "meanAmount": 0.0, "other": {"anies": [{"value": "0.0", "module": "A1", "scenario": "Standard scenario"}, {"value": "0.0", "module": "A2", "scenario": "Standard scenario"}, {"value": "3.6E-4", "module": "A3", "scenario": "Standard scenario"}, {"value": "0.0", "module": "A4", "scenario": "Standard scenario"}, {"value": "0.0", "module": "A5", "scenario": "Standard scenario"}, {"value": "0.0", "module": "B1", "scenario": "Standard scenario"}, {"value": "0.0", "module": "B2", "scenario": "Standard scenario"}, {"value": "0.0", "module": "B3", "scenario": "Standard scenario"}, {"value": "0.0", "module": "B4", "scenario": "Standard scenario"}, {"value": "0.0", "module": "B5", "scenario": "Standard scenario"}, {"value": "0.0", "module": "B6", "scenario": "Standard scenario"}, {"value": "0.0", "module": "B7", "scenario": "Standard scenario"}, {"value": "0.0", "module": "C1", "scenario": "Standard scenario"}, {"value": "0.0", "module": "C2", "scenario": "Standard scenario"}, {"value": "0.0", "module": "C3", "scenario": "Standard scenario"}, {"value": "0.0", "module": "C4", "scenario": "Standard scenario"}, {"value": "0.653", "module": "D", "scenario": "Standard scenario"}, {"name": "referenceToUnitGroupDataSet", "value": {"shortDescription": [{"value": "MJ", "lang": "en"}], "type": "unit group data set", "refObjectId": "93a60a57-a3c8-11da-a746-0800200c9a66", "version": "03.00.000", "uri": "../unitgroups/93a60a57-a3c8-11da-a746-0800200c9a66.xml"}}]}, "flowProperties": [], "typeOfFlow": "Other flow", "classification": {"classHierarchy": "Größen / Umweltliche Größen / EPD EN 15804 / LCI Indikatoren", "name": "GaBiCategories"}}, {"dataSetInternalID": 4, "referenceToFlowDataSet": {"shortDescription": [{"value": "Exported thermal energy (EET)", "lang": "en"}, {"value": "Exportierte thermische Energie (EET)", "lang": "de"}, {"value": "Energía exportada termal (EET)", "lang": "es"}], "type": "flow data set", "refObjectId": "98daf38a-7a79-46d3-9a37-2b7bd0955810", "version": "30.00.000", "uri": "../flows/98daf38a-7a79-46d3-9a37-2b7bd0955810.xml"}, "exchange direction": "OUTPUT", "meanAmount": 0.0, "other": {"anies": [{"value": "0.0", "module": "A1", "scenario": "Standard scenario"}, {"value": "0.0", "module": "A2", "scenario": "Standard scenario"}, {"value": "6.2E-4", "module": "A3", "scenario": "Standard scenario"}, {"value": "0.0", "module": "A4", "scenario": "Standard scenario"}, {"value": "0.0", "module": "A5", "scenario": "Standard scenario"}, {"value": "0.0", "module": "B1", "scenario": "Standard scenario"}, {"value": "0.0", "module": "B2", "scenario": "Standard scenario"}, {"value": "0.0", "module": "B3", "scenario": "Standard scenario"}, {"value": "0.0", "module": "B4", "scenario": "Standard scenario"}, {"value": "0.0", "module": "B5", "scenario": "Standard scenario"}, {"value": "0.0", "module": "B6", "scenario": "Standard scenario"}, {"value": "0.0", "module": "B7", "scenario": "Standard scenario"}, {"value": "0.0", "module": "C1", "scenario": "Standard scenario"}, {"value": "0.0", "module": "C2", "scenario": "Standard scenario"}, {"value": "0.0", "module": "C3", "scenario": "Standard scenario"}, {"value": "0.0", "module": "C4", "scenario": "Standard scenario"}, {"value": "1.12", "module": "D", "scenario": "Standard scenario"}, {"name": "referenceToUnitGroupDataSet", "value": {"shortDescription": [{"value": "MJ", "lang": "en"}], "type": "unit group data set", "refObjectId": "93a60a57-a3c8-11da-a746-0800200c9a66", "version": "03.00.000", "uri": "../unitgroups/93a60a57-a3c8-11da-a746-0800200c9a66.xml"}}]}, "flowProperties": [], "typeOfFlow": "Other flow", "classification": {"classHierarchy": "Größen / Umweltliche Größen / EPD EN 15804 / LCI Indikatoren", "name": "GaBiCategories"}}, {"dataSetInternalID": 5, "referenceToFlowDataSet": {"shortDescription": [{"value": "Use of net fresh water (FW)", "lang": "en"}, {"value": "Einsatz von Süßwasserressourcen (FW)", "lang": "de"}, {"value": "Uso neto de recursos de agua dulce (FW)", "lang": "es"}], "type": "flow data set", "refObjectId": "3cf952c8-f3a4-461d-8c96-96456ca62246", "version": "30.00.000", "uri": "../flows/3cf952c8-f3a4-461d-8c96-96456ca62246.xml"}, "exchange direction": "INPUT", "meanAmount": 0.0, "other": {"anies": [{"value": "1.61", "module": "A1", "scenario": "Standard scenario"}, {"value": "2.06E-4", "module": "A2", "scenario": "Standard scenario"}, {"value": "0.0498", "module": "A3", "scenario": "Standard scenario"}, {"value": "0.00119", "module": "A4", "scenario": "Standard scenario"}, {"value": "2.92E-4", "module": "A5", "scenario": "Standard scenario"}, {"value": "0.0", "module": "B1", "scenario": "Standard scenario"}, {"value": "0.0", "module": "B2", "scenario": "Standard scenario"}, {"value": "0.0", "module": "B3", "scenario": "Standard scenario"}, {"value": "0.0", "module": "B4", "scenario": "Standard scenario"}, {"value": "0.0", "module": "B5", "scenario": "Standard scenario"}, {"value": "4.69", "module": "B6", "scenario": "Standard scenario"}, {"value": "0.0", "module": "B7", "scenario": "Standard scenario"}, {"value": "0.0", "module": "C1", "scenario": "Standard scenario"}, {"value": "1.71E-4", "module": "C2", "scenario": "Standard scenario"}, {"value": "0.00166", "module": "C3", "scenario": "Standard scenario"}, {"value": "7.46E-5", "module": "C4", "scenario": "Standard scenario"}, {"value": "-0.019", "module": "D", "scenario": "Standard scenario"}, {"name": "referenceToUnitGroupDataSet", "value": {"shortDescription": [{"value": "m3", "lang": "en"}], "type": "unit group data set", "refObjectId": "cd950537-0a98-4044-9ba7-9f9a68d0a504", "version": "30.00.000", "uri": "../unitgroups/cd950537-0a98-4044-9ba7-9f9a68d0a504.xml"}}]}, "flowProperties": [], "typeOfFlow": "Other flow", "classification": {"classHierarchy": "Größen / Umweltliche Größen / EPD EN 15804 / LCI Indikatoren", "name": "GaBiCategories"}}, {"dataSetInternalID": 6, "referenceToFlowDataSet": {"shortDescription": [{"value": "Hazardous waste disposed (HWD)", "lang": "en"}, {"value": "Gefährlicher Abfall zur Deponie (HWD)", "lang": "de"}, {"value": "Residuos peligrosos eliminados (HWD)", "lang": "es"}], "type": "flow data set", "refObjectId": "430f9e0f-59b2-46a0-8e0d-55e0e84948fc", "version": "30.00.000", "uri": "../flows/430f9e0f-59b2-46a0-8e0d-55e0e84948fc.xml"}, "exchange direction": "OUTPUT", "meanAmount": 0.0, "other": {"anies": [{"value": "0.0331", "module": "A1", "scenario": "Standard scenario"}, {"value": "5.44E-6", "module": "A2", "scenario": "Standard scenario"}, {"value": "6.55E-5", "module": "A3", "scenario": "Standard scenario"}, {"value": "3.15E-5", "module": "A4", "scenario": "Standard scenario"}, {"value": "3.28E-6", "module": "A5", "scenario": "Standard scenario"}, {"value": "0.0", "module": "B1", "scenario": "Standard scenario"}, {"value": "0.0", "module": "B2", "scenario": "Standard scenario"}, {"value": "0.0", "module": "B3", "scenario": "Standard scenario"}, {"value": "0.0", "module": "B4", "scenario": "Standard scenario"}, {"value": "0.0", "module": "B5", "scenario": "Standard scenario"}, {"value": "0.0104", "module": "B6", "scenario": "Standard scenario"}, {"value": "0.0", "module": "B7", "scenario": "Standard scenario"}, {"value": "0.0", "module": "C1", "scenario": "Standard scenario"}, {"value": "4.51E-6", "module": "C2", "scenario": "Standard scenario"}, {"value": "1.63E-4", "module": "C3", "scenario": "Standard scenario"}, {"value": "3.14E-7", "module": "C4", "scenario": "Standard scenario"}, {"value": "-8.89E-5", "module": "D", "scenario": "Standard scenario"}, {"name": "referenceToUnitGroupDataSet", "value": {"shortDescription": [{"value": "kg", "lang": "en"}], "type": "unit group data set", "refObjectId": "ad38d542-3fe9-439d-9b95-2f5f7752acaf", "version": "30.00.000", "uri": "../unitgroups/ad38d542-3fe9-439d-9b95-2f5f7752acaf.xml"}}]}, "flowProperties": [], "typeOfFlow": "Other flow", "classification": {"classHierarchy": "Größen / Umweltliche Größen / EPD EN 15804 / LCI Indikatoren", "name": "GaBiCategories"}}, {"dataSetInternalID": 7, "referenceToFlowDataSet": {"shortDescription": [{"value": "Materials for energy recovery (MER)", "lang": "en"}, {"value": "Stoffe für die Energierückgewinnung (MER)", "lang": "de"}, {"value": "Materiales para valorización energética (recuperación de energía) (MER)", "lang": "es"}], "type": "flow data set", "refObjectId": "59a9181c-3aaf-46ee-8b13-2b3723b6e447", "version": "30.00.000", "uri": "../flows/59a9181c-3aaf-46ee-8b13-2b3723b6e447.xml"}, "exchange direction": "OUTPUT", "meanAmount": 0.0, "other": {"anies": [{"value": "0.0", "module": "A1", "scenario": "Standard scenario"}, {"value": "0.0", "module": "A2", "scenario": "Standard scenario"}, {"value": "0.0", "module": "A3", "scenario": "Standard scenario"}, {"value": "0.0", "module": "A4", "scenario": "Standard scenario"}, {"value": "0.0", "module": "A5", "scenario": "Standard scenario"}, {"value": "0.0", "module": "B1", "scenario": "Standard scenario"}, {"value": "0.0", "module": "B2", "scenario": "Standard scenario"}, {"value": "0.0", "module": "B3", "scenario": "Standard scenario"}, {"value": "0.0", "module": "B4", "scenario": "Standard scenario"}, {"value": "0.0", "module": "B5", "scenario": "Standard scenario"}, {"value": "0.0", "module": "B6", "scenario": "Standard scenario"}, {"value": "0.0", "module": "B7", "scenario": "Standard scenario"}, {"value": "0.0", "module": "C1", "scenario": "Standard scenario"}, {"value": "0.0", "module": "C2", "scenario": "Standard scenario"}, {"value": "0.0", "module": "C3", "scenario": "Standard scenario"}, {"value": "0.0", "module": "C4", "scenario": "Standard scenario"}, {"value": "0.0", "module": "D", "scenario": "Standard scenario"}, {"name": "referenceToUnitGroupDataSet", "value": {"shortDescription": [{"value": "kg", "lang": "en"}], "type": "unit group data set", "refObjectId": "ad38d542-3fe9-439d-9b95-2f5f7752acaf", "version": "30.00.000", "uri": "../unitgroups/ad38d542-3fe9-439d-9b95-2f5f7752acaf.xml"}}]}, "flowProperties": [], "typeOfFlow": "Other flow", "classification": {"classHierarchy": "Größen / Umweltliche Größen / EPD EN 15804 / LCI Indikatoren", "name": "GaBiCategories"}}, {"dataSetInternalID": 8, "referenceToFlowDataSet": {"shortDescription": [{"value": "Materials for recycling (MFR)", "lang": "en"}, {"value": "Stoffe zum Recycling (MFR)", "lang": "de"}, {"value": "Materiales para el reciclaje (MFR)", "lang": "es"}], "type": "flow data set", "refObjectId": "d7fe48a5-4103-49c8-9aae-b0b5dfdbd6ae", "version": "30.00.000", "uri": "../flows/d7fe48a5-4103-49c8-9aae-b0b5dfdbd6ae.xml"}, "exchange direction": "OUTPUT", "meanAmount": 0.0, "other": {"anies": [{"value": "0.0", "module": "A1", "scenario": "Standard scenario"}, {"value": "0.0", "module": "A2", "scenario": "Standard scenario"}, {"value": "0.0", "module": "A3", "scenario": "Standard scenario"}, {"value": "0.0", "module": "A4", "scenario": "Standard scenario"}, {"value": "0.554", "module": "A5", "scenario": "Standard scenario"}, {"value": "0.0", "module": "B1", "scenario": "Standard scenario"}, {"value": "0.0", "module": "B2", "scenario": "Standard scenario"}, {"value": "0.0", "module": "B3", "scenario": "Standard scenario"}, {"value": "0.0", "module": "B4", "scenario": "Standard scenario"}, {"value": "0.0", "module": "B5", "scenario": "Standard scenario"}, {"value": "0.0", "module": "B6", "scenario": "Standard scenario"}, {"value": "0.0", "module": "B7", "scenario": "Standard scenario"}, {"value": "0.0", "module": "C1", "scenario": "Standard scenario"}, {"value": "0.0", "module": "C2", "scenario": "Standard scenario"}, {"value": "2.22", "module": "C3", "scenario": "Standard scenario"}, {"value": "0.0", "module": "C4", "scenario": "Standard scenario"}, {"value": "0.0", "module": "D", "scenario": "Standard scenario"}, {"name": "referenceToUnitGroupDataSet", "value": {"shortDescription": [{"value": "kg", "lang": "en"}], "type": "unit group data set", "refObjectId": "ad38d542-3fe9-439d-9b95-2f5f7752acaf", "version": "30.00.000", "uri": "../unitgroups/ad38d542-3fe9-439d-9b95-2f5f7752acaf.xml"}}]}, "flowProperties": [], "typeOfFlow": "Other flow", "classification": {"classHierarchy": "Größen / Umweltliche Größen / EPD EN 15804 / LCI Indikatoren", "name": "GaBiCategories"}}, {"dataSetInternalID": 9, "referenceToFlowDataSet": {"shortDescription": [{"value": "Non-hazardous waste disposed (NHWD)", "lang": "en"}, {"value": "Entsorgter nicht gefährlicher Abfall (NHWD)", "lang": "de"}, {"value": "Residuos no peligrosos eliminados (NHWD)", "lang": "es"}], "type": "flow data set", "refObjectId": "b29ef66b-e286-4afa-949f-62f1a7b4d7fa", "version": "30.00.000", "uri": "../flows/b29ef66b-e286-4afa-949f-62f1a7b4d7fa.xml"}, "exchange direction": "OUTPUT", "meanAmount": 0.0, "other": {"anies": [{"value": "23.3", "module": "A1", "scenario": "Standard scenario"}, {"value": "0.0564", "module": "A2", "scenario": "Standard scenario"}, {"value": "0.217", "module": "A3", "scenario": "Standard scenario"}, {"value": "0.326", "module": "A4", "scenario": "Standard scenario"}, {"value": "0.215", "module": "A5", "scenario": "Standard scenario"}, {"value": "0.0", "module": "B1", "scenario": "Standard scenario"}, {"value": "0.0", "module": "B2", "scenario": "Standard scenario"}, {"value": "0.0", "module": "B3", "scenario": "Standard scenario"}, {"value": "0.0", "module": "B4", "scenario": "Standard scenario"}, {"value": "0.0", "module": "B5", "scenario": "Standard scenario"}, {"value": "23.7", "module": "B6", "scenario": "Standard scenario"}, {"value": "0.0", "module": "B7", "scenario": "Standard scenario"}, {"value": "0.0", "module": "C1", "scenario": "Standard scenario"}, {"value": "0.0468", "module": "C2", "scenario": "Standard scenario"}, {"value": "0.0635", "module": "C3", "scenario": "Standard scenario"}, {"value": "0.261", "module": "C4", "scenario": "Standard scenario"}, {"value": "0.592", "module": "D", "scenario": "Standard scenario"}, {"name": "referenceToUnitGroupDataSet", "value": {"shortDescription": [{"value": "kg", "lang": "en"}], "type": "unit group data set", "refObjectId": "ad38d542-3fe9-439d-9b95-2f5f7752acaf", "version": "30.00.000", "uri": "../unitgroups/ad38d542-3fe9-439d-9b95-2f5f7752acaf.xml"}}]}, "flowProperties": [], "typeOfFlow": "Other flow", "classification": {"classHierarchy": "Größen / Umweltliche Größen / EPD EN 15804 / LCI Indikatoren", "name": "GaBiCategories"}}, {"dataSetInternalID": 10, "referenceToFlowDataSet": {"shortDescription": [{"value": "Use of non renewable secondary fuels (NRSF)", "lang": "en"}, {"value": "Nicht erneuerbare Sekundärbrennstoffe (NRSF)", "lang": "de"}, {"value": "Uso de combustibles secundarios no renovables (NRSF)", "lang": "es"}], "type": "flow data set", "refObjectId": "89def144-d39a-4287-b86f-efde453ddcb2", "version": "30.00.000", "uri": "../flows/89def144-d39a-4287-b86f-efde453ddcb2.xml"}, "exchange direction": "INPUT", "meanAmount": 0.0, "other": {"anies": [{"value": "0.0", "module": "A1", "scenario": "Standard scenario"}, {"value": "0.0", "module": "A2", "scenario": "Standard scenario"}, {"value": "0.0", "module": "A3", "scenario": "Standard scenario"}, {"value": "0.0", "module": "A4", "scenario": "Standard scenario"}, {"value": "0.0", "module": "A5", "scenario": "Standard scenario"}, {"value": "0.0", "module": "B1", "scenario": "Standard scenario"}, {"value": "0.0", "module": "B2", "scenario": "Standard scenario"}, {"value": "0.0", "module": "B3", "scenario": "Standard scenario"}, {"value": "0.0", "module": "B4", "scenario": "Standard scenario"}, {"value": "0.0", "module": "B5", "scenario": "Standard scenario"}, {"value": "0.0", "module": "B6", "scenario": "Standard scenario"}, {"value": "0.0", "module": "B7", "scenario": "Standard scenario"}, {"value": "0.0", "module": "C1", "scenario": "Standard scenario"}, {"value": "0.0", "module": "C2", "scenario": "Standard scenario"}, {"value": "0.0", "module": "C3", "scenario": "Standard scenario"}, {"value": "0.0", "module": "C4", "scenario": "Standard scenario"}, {"value": "0.0", "module": "D", "scenario": "Standard scenario"}, {"name": "referenceToUnitGroupDataSet", "value": {"shortDescription": [{"value": "MJ", "lang": "en"}], "type": "unit group data set", "refObjectId": "93a60a57-a3c8-11da-a746-0800200c9a66", "version": "03.00.000", "uri": "../unitgroups/93a60a57-a3c8-11da-a746-0800200c9a66.xml"}}]}, "flowProperties": [], "typeOfFlow": "Other flow", "classification": {"classHierarchy": "Größen / Umweltliche Größen / EPD EN 15804 / LCI Indikatoren", "name": "GaBiCategories"}}, {"dataSetInternalID": 11, "referenceToFlowDataSet": {"shortDescription": [{"value": "Use of non renewable primary energy (PENRE)", "lang": "en"}, {"value": "Nicht-erneuerbare Primärenergie als Energieträger (PENRE)", "lang": "de"}, {"value": "Uso de energía primaria no renovable, excluyendo los recursos de energía primaria no renovable utilizada como materia prima (PENRE)", "lang": "es"}], "type": "flow data set", "refObjectId": "ac857178-2b45-46ec-892a-a9a4332f0372", "version": "38.00.000", "uri": "../flows/ac857178-2b45-46ec-892a-a9a4332f0372.xml"}, "exchange direction": "INPUT", "meanAmount": 0.0, "other": {"anies": [{"value": "2010.0", "module": "A1", "scenario": "Standard scenario"}, {"value": "0.855", "module": "A2", "scenario": "Standard scenario"}, {"value": "62.9", "module": "A3", "scenario": "Standard scenario"}, {"value": "4.94", "module": "A4", "scenario": "Standard scenario"}, {"value": "0.548", "module": "A5", "scenario": "Standard scenario"}, {"value": "0.0", "module": "B1", "scenario": "Standard scenario"}, {"value": "0.0", "module": "B2", "scenario": "Standard scenario"}, {"value": "0.0", "module": "B3", "scenario": "Standard scenario"}, {"value": "0.0", "module": "B4", "scenario": "Standard scenario"}, {"value": "0.0", "module": "B5", "scenario": "Standard scenario"}, {"value": "5930.0", "module": "B6", "scenario": "Standard scenario"}, {"value": "0.0", "module": "B7", "scenario": "Standard scenario"}, {"value": "0.0", "module": "C1", "scenario": "Standard scenario"}, {"value": "0.709", "module": "C2", "scenario": "Standard scenario"}, {"value": "1.35", "module": "C3", "scenario": "Standard scenario"}, {"value": "0.0652", "module": "C4", "scenario": "Standard scenario"}, {"value": "26.7", "module": "D", "scenario": "Standard scenario"}, {"name": "referenceToUnitGroupDataSet", "value": {"shortDescription": [{"value": "MJ", "lang": "en"}], "type": "unit group data set", "refObjectId": "93a60a57-a3c8-11da-a746-0800200c9a66", "version": "03.00.000", "uri": "../unitgroups/93a60a57-a3c8-11da-a746-0800200c9a66.xml"}}]}, "flowProperties": [], "typeOfFlow": "Other flow", "classification": {"classHierarchy": "Quantities", "name": "GaBiCategories"}}, {"dataSetInternalID": 12, "referenceToFlowDataSet": {"shortDescription": [{"value": "Use of non renewable primary energy resources used as raw materials (PENRM)", "lang": "en"}, {"value": "Nicht-erneuerbare Primärenergie zur stofflichen Nutzung (PENRM)", "lang": "de"}, {"value": "Uso de la energía primaria no renovable utilizada como materia prima (PENRM)", "lang": "es"}], "type": "flow data set", "refObjectId": "1421caa0-679d-4bf4-b282-0eb850ccae27", "version": "38.00.000", "uri": "../flows/1421caa0-679d-4bf4-b282-0eb850ccae27.xml"}, "exchange direction": "INPUT", "meanAmount": 0.0, "other": {"anies": [{"value": "8.53", "module": "A1", "scenario": "Standard scenario"}, {"value": "0.0", "module": "A2", "scenario": "Standard scenario"}, {"value": "0.727", "module": "A3", "scenario": "Standard scenario"}, {"value": "0.0", "module": "A4", "scenario": "Standard scenario"}, {"value": "0.0", "module": "A5", "scenario": "Standard scenario"}, {"value": "0.0", "module": "B1", "scenario": "Standard scenario"}, {"value": "0.0", "module": "B2", "scenario": "Standard scenario"}, {"value": "0.0", "module": "B3", "scenario": "Standard scenario"}, {"value": "0.0", "module": "B4", "scenario": "Standard scenario"}, {"value": "0.0", "module": "B5", "scenario": "Standard scenario"}, {"value": "0.0", "module": "B6", "scenario": "Standard scenario"}, {"value": "0.0", "module": "B7", "scenario": "Standard scenario"}, {"value": "0.0", "module": "C1", "scenario": "Standard scenario"}, {"value": "0.0", "module": "C2", "scenario": "Standard scenario"}, {"value": "0.0", "module": "C3", "scenario": "Standard scenario"}, {"value": "0.0", "module": "C4", "scenario": "Standard scenario"}, {"value": "-0.0171", "module": "D", "scenario": "Standard scenario"}, {"name": "referenceToUnitGroupDataSet", "value": {"shortDescription": [{"value": "MJ", "lang": "en"}], "type": "unit group data set", "refObjectId": "93a60a57-a3c8-11da-a746-0800200c9a66", "version": "03.00.000", "uri": "../unitgroups/93a60a57-a3c8-11da-a746-0800200c9a66.xml"}}]}, "flowProperties": [], "typeOfFlow": "Other flow", "classification": {"classHierarchy": "Quantities", "name": "GaBiCategories"}}, {"dataSetInternalID": 13, "referenceToFlowDataSet": {"shortDescription": [{"value": "Total use of non-renewable primary energy resources (PENRT)", "lang": "en"}, {"value": "Total nicht erneuerbare Primärenergie (PENRT)", "lang": "de"}, {"value": "Uso total de la energía primaria no renovable (energía primaria y recursos de energía primaria renovable utilizada como materia prima) (PENRT)", "lang": "es"}], "type": "flow data set", "refObjectId": "06159210-646b-4c8d-8583-da9b3b95a6c1", "version": "30.00.000", "uri": "../flows/06159210-646b-4c8d-8583-da9b3b95a6c1.xml"}, "exchange direction": "INPUT", "meanAmount": 0.0, "other": {"anies": [{"value": "2020.0", "module": "A1", "scenario": "Standard scenario"}, {"value": "0.855", "module": "A2", "scenario": "Standard scenario"}, {"value": "63.6", "module": "A3", "scenario": "Standard scenario"}, {"value": "4.94", "module": "A4", "scenario": "Standard scenario"}, {"value": "0.548", "module": "A5", "scenario": "Standard scenario"}, {"value": "0.0", "module": "B1", "scenario": "Standard scenario"}, {"value": "0.0", "module": "B2", "scenario": "Standard scenario"}, {"value": "0.0", "module": "B3", "scenario": "Standard scenario"}, {"value": "0.0", "module": "B4", "scenario": "Standard scenario"}, {"value": "0.0", "module": "B5", "scenario": "Standard scenario"}, {"value": "5930.0", "module": "B6", "scenario": "Standard scenario"}, {"value": "0.0", "module": "B7", "scenario": "Standard scenario"}, {"value": "0.0", "module": "C1", "scenario": "Standard scenario"}, {"value": "0.709", "module": "C2", "scenario": "Standard scenario"}, {"value": "1.35", "module": "C3", "scenario": "Standard scenario"}, {"value": "0.0652", "module": "C4", "scenario": "Standard scenario"}, {"value": "26.7", "module": "D", "scenario": "Standard scenario"}, {"name": "referenceToUnitGroupDataSet", "value": {"shortDescription": [{"value": "MJ", "lang": "en"}], "type": "unit group data set", "refObjectId": "93a60a57-a3c8-11da-a746-0800200c9a66", "version": "03.00.000", "uri": "../unitgroups/93a60a57-a3c8-11da-a746-0800200c9a66.xml"}}]}, "flowProperties": [], "typeOfFlow": "Other flow", "classification": {"classHierarchy": "Größen / Umweltliche Größen / EPD EN 15804 / LCI Indikatoren", "name": "GaBiCategories"}}, {"dataSetInternalID": 14, "referenceToFlowDataSet": {"shortDescription": [{"value": "Use of renewable primary energy (PERE)", "lang": "en"}, {"value": "Erneuerbare Primärenergie als Energieträger (PERE)", "lang": "de"}, {"value": "Uso de energía primaria renovable excluyendo los recursos de energía primaria renovable utilizada como materia prima (PERE)", "lang": "es"}], "type": "flow data set", "refObjectId": "20f32be5-0398-4288-9b6d-accddd195317", "version": "38.00.000", "uri": "../flows/20f32be5-0398-4288-9b6d-accddd195317.xml"}, "exchange direction": "INPUT", "meanAmount": 0.0, "other": {"anies": [{"value": "281.0", "module": "A1", "scenario": "Standard scenario"}, {"value": "0.0121", "module": "A2", "scenario": "Standard scenario"}, {"value": "15.9", "module": "A3", "scenario": "Standard scenario"}, {"value": "0.0697", "module": "A4", "scenario": "Standard scenario"}, {"value": "0.0214", "module": "A5", "scenario": "Standard scenario"}, {"value": "0.0", "module": "B1", "scenario": "Standard scenario"}, {"value": "0.0", "module": "B2", "scenario": "Standard scenario"}, {"value": "0.0", "module": "B3", "scenario": "Standard scenario"}, {"value": "0.0", "module": "B4", "scenario": "Standard scenario"}, {"value": "0.0", "module": "B5", "scenario": "Standard scenario"}, {"value": "1300.0", "module": "B6", "scenario": "Standard scenario"}, {"value": "0.0", "module": "B7", "scenario": "Standard scenario"}, {"value": "0.0", "module": "C1", "scenario": "Standard scenario"}, {"value": "0.01", "module": "C2", "scenario": "Standard scenario"}, {"value": "0.139", "module": "C3", "scenario": "Standard scenario"}, {"value": "0.0029", "module": "C4", "scenario": "Standard scenario"}, {"value": "-1.86", "module": "D", "scenario": "Standard scenario"}, {"name": "referenceToUnitGroupDataSet", "value": {"shortDescription": [{"value": "MJ", "lang": "en"}], "type": "unit group data set", "refObjectId": "93a60a57-a3c8-11da-a746-0800200c9a66", "version": "03.00.000", "uri": "../unitgroups/93a60a57-a3c8-11da-a746-0800200c9a66.xml"}}]}, "flowProperties": [], "typeOfFlow": "Other flow", "classification": {"classHierarchy": "Quantities", "name": "GaBiCategories"}}, {"dataSetInternalID": 15, "referenceToFlowDataSet": {"shortDescription": [{"value": "Use of renewable primary energy resources used as raw materials (PERM)", "lang": "en"}, {"value": "Erneuerbare Primärenergie zur stofflichen Nutzung (PERM)", "lang": "de"}, {"value": "Uso de energía primaria renovable utilizada como materia prima (PERM)", "lang": "es"}], "type": "flow data set", "refObjectId": "fb3ec0de-548d-4508-aea5-00b73bf6f702", "version": "38.00.000", "uri": "../flows/fb3ec0de-548d-4508-aea5-00b73bf6f702.xml"}, "exchange direction": "INPUT", "meanAmount": 0.0, "other": {"anies": [{"value": "0.0", "module": "A1", "scenario": "Standard scenario"}, {"value": "0.0", "module": "A2", "scenario": "Standard scenario"}, {"value": "11.5", "module": "A3", "scenario": "Standard scenario"}, {"value": "0.0", "module": "A4", "scenario": "Standard scenario"}, {"value": "0.0", "module": "A5", "scenario": "Standard scenario"}, {"value": "0.0", "module": "B1", "scenario": "Standard scenario"}, {"value": "0.0", "module": "B2", "scenario": "Standard scenario"}, {"value": "0.0", "module": "B3", "scenario": "Standard scenario"}, {"value": "0.0", "module": "B4", "scenario": "Standard scenario"}, {"value": "0.0", "module": "B5", "scenario": "Standard scenario"}, {"value": "0.0", "module": "B6", "scenario": "Standard scenario"}, {"value": "0.0", "module": "B7", "scenario": "Standard scenario"}, {"value": "0.0", "module": "C1", "scenario": "Standard scenario"}, {"value": "0.0", "module": "C2", "scenario": "Standard scenario"}, {"value": "0.0", "module": "C3", "scenario": "Standard scenario"}, {"value": "0.0", "module": "C4", "scenario": "Standard scenario"}, {"value": "0.0", "module": "D", "scenario": "Standard scenario"}, {"name": "referenceToUnitGroupDataSet", "value": {"shortDescription": [{"value": "MJ", "lang": "en"}], "type": "unit group data set", "refObjectId": "93a60a57-a3c8-11da-a746-0800200c9a66", "version": "03.00.000", "uri": "../unitgroups/93a60a57-a3c8-11da-a746-0800200c9a66.xml"}}]}, "flowProperties": [], "typeOfFlow": "Other flow", "classification": {"classHierarchy": "Quantities", "name": "GaBiCategories"}}, {"dataSetInternalID": 16, "referenceToFlowDataSet": {"shortDescription": [{"value": "Total use of renewable primary energy resources (PERT)", "lang": "en"}, {"value": "Total erneuerbare Primärenergie (PERT)", "lang": "de"}, {"value": "Uso total de la energía primaria renovable (energía primaria y recursos de energía primaria renovable utilizada como materia prima) (PERT)", "lang": "es"}], "type": "flow data set", "refObjectId": "53f97275-fa8a-4cdd-9024-65936002acd0", "version": "30.00.000", "uri": "../flows/53f97275-fa8a-4cdd-9024-65936002acd0.xml"}, "exchange direction": "INPUT", "meanAmount": 0.0, "other": {"anies": [{"value": "281.0", "module": "A1", "scenario": "Standard scenario"}, {"value": "0.0121", "module": "A2", "scenario": "Standard scenario"}, {"value": "27.4", "module": "A3", "scenario": "Standard scenario"}, {"value": "0.0697", "module": "A4", "scenario": "Standard scenario"}, {"value": "0.0214", "module": "A5", "scenario": "Standard scenario"}, {"value": "0.0", "module": "B1", "scenario": "Standard scenario"}, {"value": "0.0", "module": "B2", "scenario": "Standard scenario"}, {"value": "0.0", "module": "B3", "scenario": "Standard scenario"}, {"value": "0.0", "module": "B4", "scenario": "Standard scenario"}, {"value": "0.0", "module": "B5", "scenario": "Standard scenario"}, {"value": "1300.0", "module": "B6", "scenario": "Standard scenario"}, {"value": "0.0", "module": "B7", "scenario": "Standard scenario"}, {"value": "0.0", "module": "C1", "scenario": "Standard scenario"}, {"value": "0.01", "module": "C2", "scenario": "Standard scenario"}, {"value": "0.139", "module": "C3", "scenario": "Standard scenario"}, {"value": "0.0029", "module": "C4", "scenario": "Standard scenario"}, {"value": "-1.86", "module": "D", "scenario": "Standard scenario"}, {"name": "referenceToUnitGroupDataSet", "value": {"shortDescription": [{"value": "MJ", "lang": "en"}], "type": "unit group data set", "refObjectId": "93a60a57-a3c8-11da-a746-0800200c9a66", "version": "03.00.000", "uri": "../unitgroups/93a60a57-a3c8-11da-a746-0800200c9a66.xml"}}]}, "flowProperties": [], "typeOfFlow": "Other flow", "classification": {"classHierarchy": "Größen / Umweltliche Größen / EPD EN 15804 / LCI Indikatoren", "name": "GaBiCategories"}}, {"dataSetInternalID": 17, "referenceToFlowDataSet": {"shortDescription": [{"value": "Use of renewable secondary fuels (RSF)", "lang": "en"}, {"value": "Erneuerbare Sekundärbrennstoffe (RSF)", "lang": "de"}, {"value": "Uso de combustibles secundarios renovables (RSF)", "lang": "es"}], "type": "flow data set", "refObjectId": "64333088-a55f-4aa2-9a31-c10b07816787", "version": "30.00.000", "uri": "../flows/64333088-a55f-4aa2-9a31-c10b07816787.xml"}, "exchange direction": "INPUT", "meanAmount": 0.0, "other": {"anies": [{"value": "0.0", "module": "A1", "scenario": "Standard scenario"}, {"value": "0.0", "module": "A2", "scenario": "Standard scenario"}, {"value": "0.0", "module": "A3", "scenario": "Standard scenario"}, {"value": "0.0", "module": "A4", "scenario": "Standard scenario"}, {"value": "0.0", "module": "A5", "scenario": "Standard scenario"}, {"value": "0.0", "module": "B1", "scenario": "Standard scenario"}, {"value": "0.0", "module": "B2", "scenario": "Standard scenario"}, {"value": "0.0", "module": "B3", "scenario": "Standard scenario"}, {"value": "0.0", "module": "B4", "scenario": "Standard scenario"}, {"value": "0.0", "module": "B5", "scenario": "Standard scenario"}, {"value": "0.0", "module": "B6", "scenario": "Standard scenario"}, {"value": "0.0", "module": "B7", "scenario": "Standard scenario"}, {"value": "0.0", "module": "C1", "scenario": "Standard scenario"}, {"value": "0.0", "module": "C2", "scenario": "Standard scenario"}, {"value": "0.0", "module": "C3", "scenario": "Standard scenario"}, {"value": "0.0", "module": "C4", "scenario": "Standard scenario"}, {"value": "0.0", "module": "D", "scenario": "Standard scenario"}, {"name": "referenceToUnitGroupDataSet", "value": {"shortDescription": [{"value": "MJ", "lang": "en"}], "type": "unit group data set", "refObjectId": "93a60a57-a3c8-11da-a746-0800200c9a66", "version": "03.00.000", "uri": "../unitgroups/93a60a57-a3c8-11da-a746-0800200c9a66.xml"}}]}, "flowProperties": [], "typeOfFlow": "Other flow", "classification": {"classHierarchy": "Größen / Umweltliche Größen / EPD EN 15804 / LCI Indikatoren", "name": "GaBiCategories"}}, {"dataSetInternalID": 18, "referenceToFlowDataSet": {"shortDescription": [{"value": "Radioactive waste disposed (RWD)", "lang": "en"}, {"value": "Entsorgter radioaktiver Abfall (RWD)", "lang": "de"}, {"value": "Residuos radiactivos eliminados (RWD)", "lang": "es"}], "type": "flow data set", "refObjectId": "3449546e-52ad-4b39-b809-9fb77cea8ff6", "version": "30.00.000", "uri": "../flows/3449546e-52ad-4b39-b809-9fb77cea8ff6.xml"}, "exchange direction": "OUTPUT", "meanAmount": 0.0, "other": {"anies": [{"value": "0.0126", "module": "A1", "scenario": "Standard scenario"}, {"value": "1.95E-7", "module": "A2", "scenario": "Standard scenario"}, {"value": "8.42E-4", "module": "A3", "scenario": "Standard scenario"}, {"value": "1.13E-6", "module": "A4", "scenario": "Standard scenario"}, {"value": "5.13E-7", "module": "A5", "scenario": "Standard scenario"}, {"value": "0.0", "module": "B1", "scenario": "Standard scenario"}, {"value": "0.0", "module": "B2", "scenario": "Standard scenario"}, {"value": "0.0", "module": "B3", "scenario": "Standard scenario"}, {"value": "0.0", "module": "B4", "scenario": "Standard scenario"}, {"value": "0.0", "module": "B5", "scenario": "Standard scenario"}, {"value": "0.0425", "module": "B6", "scenario": "Standard scenario"}, {"value": "0.0", "module": "B7", "scenario": "Standard scenario"}, {"value": "0.0", "module": "C1", "scenario": "Standard scenario"}, {"value": "1.62E-7", "module": "C2", "scenario": "Standard scenario"}, {"value": "2.61E-6", "module": "C3", "scenario": "Standard scenario"}, {"value": "3.76E-8", "module": "C4", "scenario": "Standard scenario"}, {"value": "1.43E-4", "module": "D", "scenario": "Standard scenario"}, {"name": "referenceToUnitGroupDataSet", "value": {"shortDescription": [{"value": "kg", "lang": "en"}], "type": "unit group data set", "refObjectId": "ad38d542-3fe9-439d-9b95-2f5f7752acaf", "version": "30.00.000", "uri": "../unitgroups/ad38d542-3fe9-439d-9b95-2f5f7752acaf.xml"}}]}, "flowProperties": [], "typeOfFlow": "Other flow", "classification": {"classHierarchy": "Größen / Umweltliche Größen / EPD EN 15804 / LCI Indikatoren", "name": "GaBiCategories"}}, {"dataSetInternalID": 19, "referenceToFlowDataSet": {"shortDescription": [{"value": "Use of secondary material (SM)", "lang": "en"}, {"value": "Einsatz von Sekundärstoffen (SM)", "lang": "de"}, {"value": "Uso de materiales secundarios (SM)", "lang": "es"}], "type": "flow data set", "refObjectId": "c6a1f35f-2d09-4f54-8dfb-97e502e1ce92", "version": "30.00.000", "uri": "../flows/c6a1f35f-2d09-4f54-8dfb-97e502e1ce92.xml"}, "exchange direction": "INPUT", "meanAmount": 0.0, "other": {"anies": [{"value": "0.0", "module": "A1", "scenario": "Standard scenario"}, {"value": "0.0", "module": "A2", "scenario": "Standard scenario"}, {"value": "0.0", "module": "A3", "scenario": "Standard scenario"}, {"value": "0.0", "module": "A4", "scenario": "Standard scenario"}, {"value": "0.0", "module": "A5", "scenario": "Standard scenario"}, {"value": "0.0", "module": "B1", "scenario": "Standard scenario"}, {"value": "0.0", "module": "B2", "scenario": "Standard scenario"}, {"value": "0.0", "module": "B3", "scenario": "Standard scenario"}, {"value": "0.0", "module": "B4", "scenario": "Standard scenario"}, {"value": "0.0", "module": "B5", "scenario": "Standard scenario"}, {"value": "0.0", "module": "B6", "scenario": "Standard scenario"}, {"value": "0.0", "module": "B7", "scenario": "Standard scenario"}, {"value": "0.0", "module": "C1", "scenario": "Standard scenario"}, {"value": "0.0", "module": "C2", "scenario": "Standard scenario"}, {"value": "0.0", "module": "C3", "scenario": "Standard scenario"}, {"value": "0.0", "module": "C4", "scenario": "Standard scenario"}, {"value": "0.0", "module": "D", "scenario": "Standard scenario"}, {"name": "referenceToUnitGroupDataSet", "value": {"shortDescription": [{"value": "kg", "lang": "en"}], "type": "unit group data set", "refObjectId": "ad38d542-3fe9-439d-9b95-2f5f7752acaf", "version": "30.00.000", "uri": "../unitgroups/ad38d542-3fe9-439d-9b95-2f5f7752acaf.xml"}}]}, "flowProperties": [], "typeOfFlow": "Other flow", "classification": {"classHierarchy": "Größen / Umweltliche Größen / EPD EN 15804 / LCI Indikatoren", "name": "GaBiCategories"}}]}, "LCIAResults": {"LCIAResult": [{"referenceToLCIAMethodDataSet": {"shortDescription": [{"value": "Abiotic depletion potential - non-fossil resources (ADPE)", "lang": "en"}, {"value": "Potenzial für die Verknappung abiotischer Ressourcen – nicht fossile Ressourcen (ADPE)", "lang": "de"}], "type": "LCIA method data set", "refObjectId": "b2ad6494-c78d-11e6-9d9d-cec0c932ce01", "version": "01.00.011", "uri": "../lciamethods/b2ad6494-c78d-11e6-9d9d-cec0c932ce01.xml"}, "meanAmount": 0.0, "other": {"anies": [{"value": "0.0234", "module": "A1", "scenario": "Standard scenario"}, {"value": "1.87E-7", "module": "A2", "scenario": "Standard scenario"}, {"value": "2.89E-5", "module": "A3", "scenario": "Standard scenario"}, {"value": "1.08E-6", "module": "A4", "scenario": "Standard scenario"}, {"value": "2.02E-7", "module": "A5", "scenario": "Standard scenario"}, {"value": "0.0", "module": "B1", "scenario": "Standard scenario"}, {"value": "0.0", "module": "B2", "scenario": "Standard scenario"}, {"value": "0.0", "module": "B3", "scenario": "Standard scenario"}, {"value": "0.0", "module": "B4", "scenario": "Standard scenario"}, {"value": "0.0", "module": "B5", "scenario": "Standard scenario"}, {"value": "0.00313", "module": "B6", "scenario": "Standard scenario"}, {"value": "0.0", "module": "B7", "scenario": "Standard scenario"}, {"value": "0.0", "module": "C1", "scenario": "Standard scenario"}, {"value": "1.55E-7", "module": "C2", "scenario": "Standard scenario"}, {"value": "9.0E-7", "module": "C3", "scenario": "Standard scenario"}, {"value": "7.23E-9", "module": "C4", "scenario": "Standard scenario"}, {"value": "0.00346", "module": "D", "scenario": "Standard scenario"}, {"name": "referenceToUnitGroupDataSet", "value": {"shortDescription": [{"value": "kg Sb-eq.", "lang": "en"}], "type": "unit group data set", "refObjectId": "54ccd2d9-a32a-4fc2-923d-f2c8c93e89d4", "version": "30.00.000", "uri": "../unitgroups/54ccd2d9-a32a-4fc2-923d-f2c8c93e89d4.xml"}}]}}, {"referenceToLCIAMethodDataSet": {"shortDescription": [{"value": "Abiotic depletion potential - fossil resources (ADPF)", "lang": "en"}, {"value": "Potenzial für die Verknappung abiotischer Ressourcen – fossile Brennstoffe (ADPF)", "lang": "de"}], "type": "LCIA method data set", "refObjectId": "b2ad6110-c78d-11e6-9d9d-cec0c932ce01", "version": "01.00.011", "uri": "../lciamethods/b2ad6110-c78d-11e6-9d9d-cec0c932ce01.xml"}, "meanAmount": 0.0, "other": {"anies": [{"value": "1870.0", "module": "A1", "scenario": "Standard scenario"}, {"value": "0.854", "module": "A2", "scenario": "Standard scenario"}, {"value": "63.6", "module": "A3", "scenario": "Standard scenario"}, {"value": "4.93", "module": "A4", "scenario": "Standard scenario"}, {"value": "0.548", "module": "A5", "scenario": "Standard scenario"}, {"value": "0.0", "module": "B1", "scenario": "Standard scenario"}, {"value": "0.0", "module": "B2", "scenario": "Standard scenario"}, {"value": "0.0", "module": "B3", "scenario": "Standard scenario"}, {"value": "0.0", "module": "B4", "scenario": "Standard scenario"}, {"value": "0.0", "module": "B5", "scenario": "Standard scenario"}, {"value": "5930.0", "module": "B6", "scenario": "Standard scenario"}, {"value": "0.0", "module": "B7", "scenario": "Standard scenario"}, {"value": "0.0", "module": "C1", "scenario": "Standard scenario"}, {"value": "0.708", "module": "C2", "scenario": "Standard scenario"}, {"value": "1.35", "module": "C3", "scenario": "Standard scenario"}, {"value": "0.0652", "module": "C4", "scenario": "Standard scenario"}, {"value": "26.7", "module": "D", "scenario": "Standard scenario"}, {"name": "referenceToUnitGroupDataSet", "value": {"shortDescription": [{"value": "MJ", "lang": "en"}], "type": "unit group data set", "refObjectId": "93a60a57-a3c8-11da-a746-0800200c9a66", "version": "03.00.000", "uri": "../unitgroups/93a60a57-a3c8-11da-a746-0800200c9a66.xml"}}]}}, {"referenceToLCIAMethodDataSet": {"shortDescription": [{"value": "Acidification potential, Accumulated Exceedance (AP)", "lang": "en"}, {"value": "Versauerungspotenzial, kumulierte Überschreitung (AP)", "lang": "de"}], "type": "LCIA method data set", "refObjectId": "b5c611c6-def3-11e6-bf01-fe55135034f3", "version": "01.03.010", "uri": "../lciamethods/b5c611c6-def3-11e6-bf01-fe55135034f3.xml"}, "meanAmount": 0.0, "other": {"anies": [{"value": "0.909", "module": "A1", "scenario": "Standard scenario"}, {"value": "2.85E-4", "module": "A2", "scenario": "Standard scenario"}, {"value": "0.00552", "module": "A3", "scenario": "Standard scenario"}, {"value": "0.00165", "module": "A4", "scenario": "Standard scenario"}, {"value": "2.9E-4", "module": "A5", "scenario": "Standard scenario"}, {"value": "0.0", "module": "B1", "scenario": "Standard scenario"}, {"value": "0.0", "module": "B2", "scenario": "Standard scenario"}, {"value": "0.0", "module": "B3", "scenario": "Standard scenario"}, {"value": "0.0", "module": "B4", "scenario": "Standard scenario"}, {"value": "0.0", "module": "B5", "scenario": "Standard scenario"}, {"value": "1.5", "module": "B6", "scenario": "Standard scenario"}, {"value": "0.0", "module": "B7", "scenario": "Standard scenario"}, {"value": "0.0", "module": "C1", "scenario": "Standard scenario"}, {"value": "2.37E-4", "module": "C2", "scenario": "Standard scenario"}, {"value": "9.29E-4", "module": "C3", "scenario": "Standard scenario"}, {"value": "2.06E-5", "module": "C4", "scenario": "Standard scenario"}, {"value": "0.0177", "module": "D", "scenario": "Standard scenario"}, {"name": "referenceToUnitGroupDataSet", "value": {"shortDescription": [{"value": "mol H+-eq.", "lang": "en"}], "type": "unit group data set", "refObjectId": "42e089ac-92bf-4bf2-8ca1-5fc40d18f2ed", "version": "00.01.000", "uri": "../unitgroups/42e089ac-92bf-4bf2-8ca1-5fc40d18f2ed.xml"}}]}}, {"referenceToLCIAMethodDataSet": {"shortDescription": [{"value": "Eutrophication potential - freshwater (EP-freshwater)", "lang": "en"}, {"value": "Eutrophierungspotenzial - Süßwasser (EP-freshwater)", "lang": "de"}], "type": "LCIA method data set", "refObjectId": "b53ec18f-7377-4ad3-86eb-cc3f4f276b2b", "version": "01.00.011", "uri": "../lciamethods/b53ec18f-7377-4ad3-86eb-cc3f4f276b2b.xml"}, "meanAmount": 0.0, "other": {"anies": [{"value": "0.012", "module": "A1", "scenario": "Standard scenario"}, {"value": "5.93E-7", "module": "A2", "scenario": "Standard scenario"}, {"value": "5.34E-5", "module": "A3", "scenario": "Standard scenario"}, {"value": "3.43E-6", "module": "A4", "scenario": "Standard scenario"}, {"value": "7.42E-7", "module": "A5", "scenario": "Standard scenario"}, {"value": "0.0", "module": "B1", "scenario": "Standard scenario"}, {"value": "0.0", "module": "B2", "scenario": "Standard scenario"}, {"value": "0.0", "module": "B3", "scenario": "Standard scenario"}, {"value": "0.0", "module": "B4", "scenario": "Standard scenario"}, {"value": "0.0", "module": "B5", "scenario": "Standard scenario"}, {"value": "0.0259", "module": "B6", "scenario": "Standard scenario"}, {"value": "0.0", "module": "B7", "scenario": "Standard scenario"}, {"value": "0.0", "module": "C1", "scenario": "Standard scenario"}, {"value": "4.92E-7", "module": "C2", "scenario": "Standard scenario"}, {"value": "4.38E-6", "module": "C3", "scenario": "Standard scenario"}, {"value": "4.92E-8", "module": "C4", "scenario": "Standard scenario"}, {"value": "0.00112", "module": "D", "scenario": "Standard scenario"}, {"name": "referenceToUnitGroupDataSet", "value": {"shortDescription": [{"value": "kg P-eq.", "lang": "en"}], "type": "unit group data set", "refObjectId": "0429039d-a61d-4590-ba67-aa4a20a810a1", "version": "30.00.000", "uri": "../unitgroups/0429039d-a61d-4590-ba67-aa4a20a810a1.xml"}}]}}, {"referenceToLCIAMethodDataSet": {"shortDescription": [{"value": "Eutrophication potential - marine (EP-marine)", "lang": "en"}, {"value": "Eutrophierungspotenzial - Salzwasser (EP-marine)", "lang": "de"}], "type": "LCIA method data set", "refObjectId": "b5c619fa-def3-11e6-bf01-fe55135034f3", "version": "02.00.011", "uri": "../lciamethods/b5c619fa-def3-11e6-bf01-fe55135034f3.xml"}, "meanAmount": 0.0, "other": {"anies": [{"value": "0.119", "module": "A1", "scenario": "Standard scenario"}, {"value": "1.08E-4", "module": "A2", "scenario": "Standard scenario"}, {"value": "0.00128", "module": "A3", "scenario": "Standard scenario"}, {"value": "6.27E-4", "module": "A4", "scenario": "Standard scenario"}, {"value": "1.15E-4", "module": "A5", "scenario": "Standard scenario"}, {"value": "0.0", "module": "B1", "scenario": "Standard scenario"}, {"value": "0.0", "module": "B2", "scenario": "Standard scenario"}, {"value": "0.0", "module": "B3", "scenario": "Standard scenario"}, {"value": "0.0", "module": "B4", "scenario": "Standard scenario"}, {"value": "0.0", "module": "B5", "scenario": "Standard scenario"}, {"value": "0.188", "module": "B6", "scenario": "Standard scenario"}, {"value": "0.0", "module": "B7", "scenario": "Standard scenario"}, {"value": "0.0", "module": "C1", "scenario": "Standard scenario"}, {"value": "8.99E-5", "module": "C2", "scenario": "Standard scenario"}, {"value": "3.31E-4", "module": "C3", "scenario": "Standard scenario"}, {"value": "3.8E-5", "module": "C4", "scenario": "Standard scenario"}, {"value": "0.00436", "module": "D", "scenario": "Standard scenario"}, {"name": "referenceToUnitGroupDataSet", "value": {"shortDescription": [{"value": "kg N-eq.", "lang": "en"}], "type": "unit group data set", "refObjectId": "d05bb823-ecdf-4686-8c40-bf1d9257859f", "version": "00.00.003", "uri": "../unitgroups/d05bb823-ecdf-4686-8c40-bf1d9257859f.xml"}}]}}, {"referenceToLCIAMethodDataSet": {"shortDescription": [{"value": "Eutrophication potential - terrestrial (EP-terrestrial)", "lang": "en"}, {"value": "Eutrophierungspotenzial - Land (EP-terrestrial)", "lang": "de"}], "type": "LCIA method data set", "refObjectId": "b5c614d2-def3-11e6-bf01-fe55135034f3", "version": "01.02.010", "uri": "../lciamethods/b5c614d2-def3-11e6-bf01-fe55135034f3.xml"}, "meanAmount": 0.0, "other": {"anies": [{"value": "1.42", "module": "A1", "scenario": "Standard scenario"}, {"value": "0.00116", "module": "A2", "scenario": "Standard scenario"}, {"value": "0.0121", "module": "A3", "scenario": "Standard scenario"}, {"value": "0.00669", "module": "A4", "scenario": "Standard scenario"}, {"value": "0.00122", "module": "A5", "scenario": "Standard scenario"}, {"value": "0.0", "module": "B1", "scenario": "Standard scenario"}, {"value": "0.0", "module": "B2", "scenario": "Standard scenario"}, {"value": "0.0", "module": "B3", "scenario": "Standard scenario"}, {"value": "0.0", "module": "B4", "scenario": "Standard scenario"}, {"value": "0.0", "module": "B5", "scenario": "Standard scenario"}, {"value": "2.2", "module": "B6", "scenario": "Standard scenario"}, {"value": "0.0", "module": "B7", "scenario": "Standard scenario"}, {"value": "0.0", "module": "C1", "scenario": "Standard scenario"}, {"value": "9.59E-4", "module": "C2", "scenario": "Standard scenario"}, {"value": "0.00345", "module": "C3", "scenario": "Standard scenario"}, {"value": "8.73E-5", "module": "C4", "scenario": "Standard scenario"}, {"value": "0.0487", "module": "D", "scenario": "Standard scenario"}, {"name": "referenceToUnitGroupDataSet", "value": {"shortDescription": [{"value": "mol N-eq.", "lang": "en"}], "type": "unit group data set", "refObjectId": "71b4d617-0ec9-4d3f-b65e-e438940c2401", "version": "00.00.003", "uri": "../unitgroups/71b4d617-0ec9-4d3f-b65e-e438940c2401.xml"}}]}}, {"referenceToLCIAMethodDataSet": {"shortDescription": [{"value": "Potential Comparative Toxic Unit for ecosystems (ETP-fw)", "lang": "en"}, {"value": "Potenzielle Toxizitätsvergleichseinheit für Ökosysteme (ETP-fw)", "lang": "de"}], "type": "LCIA method data set", "refObjectId": "05316e7a-b254-4bea-9cf0-6bf33eb5c630", "version": "01.00.003", "uri": "../lciamethods/05316e7a-b254-4bea-9cf0-6bf33eb5c630.xml"}, "meanAmount": 0.0, "other": {"anies": [{"value": "2410.0", "module": "A1", "scenario": "Standard scenario"}, {"value": "0.63", "module": "A2", "scenario": "Standard scenario"}, {"value": "6.51", "module": "A3", "scenario": "Standard scenario"}, {"value": "3.64", "module": "A4", "scenario": "Standard scenario"}, {"value": "1.02", "module": "A5", "scenario": "Standard scenario"}, {"value": "0.0", "module": "B1", "scenario": "Standard scenario"}, {"value": "0.0", "module": "B2", "scenario": "Standard scenario"}, {"value": "0.0", "module": "B3", "scenario": "Standard scenario"}, {"value": "0.0", "module": "B4", "scenario": "Standard scenario"}, {"value": "0.0", "module": "B5", "scenario": "Standard scenario"}, {"value": "996.0", "module": "B6", "scenario": "Standard scenario"}, {"value": "0.0", "module": "B7", "scenario": "Standard scenario"}, {"value": "0.0", "module": "C1", "scenario": "Standard scenario"}, {"value": "0.522", "module": "C2", "scenario": "Standard scenario"}, {"value": "21.4", "module": "C3", "scenario": "Standard scenario"}, {"value": "1.33", "module": "C4", "scenario": "Standard scenario"}, {"value": "235.0", "module": "D", "scenario": "Standard scenario"}, {"name": "referenceToUnitGroupDataSet", "value": {"shortDescription": [{"value": "CTUe", "lang": "en"}], "type": "unit group data set", "refObjectId": "aa959ded-f1eb-4efb-9c5c-2d60be36b3e6", "version": "00.00.003", "uri": "../unitgroups/aa959ded-f1eb-4efb-9c5c-2d60be36b3e6.xml"}}]}}, {"referenceToLCIAMethodDataSet": {"shortDescription": [{"value": "Global Warming Potential - biogenic (GWP-biogenic)", "lang": "en"}, {"value": "Globales Erwärmungspotenzial - biogen (GWP-biogenic)", "lang": "de"}], "type": "LCIA method data set", "refObjectId": "a7ea186c-9749-11ed-a8fc-0242ac120002", "version": "01.00.006", "uri": "../lciamethods/a7ea186c-9749-11ed-a8fc-0242ac120002.xml"}, "meanAmount": 0.0, "other": {"anies": [{"value": "0.225", "module": "A1", "scenario": "Standard scenario"}, {"value": "1.94E-5", "module": "A2", "scenario": "Standard scenario"}, {"value": "-1.19", "module": "A3", "scenario": "Standard scenario"}, {"value": "1.12E-4", "module": "A4", "scenario": "Standard scenario"}, {"value": "1.21", "module": "A5", "scenario": "Standard scenario"}, {"value": "0.0", "module": "B1", "scenario": "Standard scenario"}, {"value": "0.0", "module": "B2", "scenario": "Standard scenario"}, {"value": "0.0", "module": "B3", "scenario": "Standard scenario"}, {"value": "0.0", "module": "B4", "scenario": "Standard scenario"}, {"value": "0.0", "module": "B5", "scenario": "Standard scenario"}, {"value": "1.43", "module": "B6", "scenario": "Standard scenario"}, {"value": "0.0", "module": "B7", "scenario": "Standard scenario"}, {"value": "0.0", "module": "C1", "scenario": "Standard scenario"}, {"value": "1.61E-5", "module": "C2", "scenario": "Standard scenario"}, {"value": "2.77E-4", "module": "C3", "scenario": "Standard scenario"}, {"value": "1.07E-5", "module": "C4", "scenario": "Standard scenario"}, {"value": "0.0129", "module": "D", "scenario": "Standard scenario"}, {"name": "referenceToUnitGroupDataSet", "value": {"shortDescription": [{"value": "kg CO2-eq.", "lang": "en"}], "type": "unit group data set", "refObjectId": "1ebf3012-d0db-4de2-aefd-ef30cedb0be1", "version": "30.00.000", "uri": "../unitgroups/1ebf3012-d0db-4de2-aefd-ef30cedb0be1.xml"}}]}}, {"referenceToLCIAMethodDataSet": {"shortDescription": [{"value": "Global Warming Potential - fossil fuels (GWP-fossil)", "lang": "en"}, {"value": "Globales Erwärmungspotenzial - fossil (GWP-fossil)", "lang": "de"}], "type": "LCIA method data set", "refObjectId": "a7ea19c0-9749-11ed-a8fc-0242ac120002", "version": "01.00.009", "uri": "../lciamethods/a7ea19c0-9749-11ed-a8fc-0242ac120002.xml"}, "meanAmount": 0.0, "other": {"anies": [{"value": "93.9", "module": "A1", "scenario": "Standard scenario"}, {"value": "0.0596", "module": "A2", "scenario": "Standard scenario"}, {"value": "0.563", "module": "A3", "scenario": "Standard scenario"}, {"value": "0.344", "module": "A4", "scenario": "Standard scenario"}, {"value": "0.0751", "module": "A5", "scenario": "Standard scenario"}, {"value": "0.0", "module": "B1", "scenario": "Standard scenario"}, {"value": "0.0", "module": "B2", "scenario": "Standard scenario"}, {"value": "0.0", "module": "B3", "scenario": "Standard scenario"}, {"value": "0.0", "module": "B4", "scenario": "Standard scenario"}, {"value": "0.0", "module": "B5", "scenario": "Standard scenario"}, {"value": "262.0", "module": "B6", "scenario": "Standard scenario"}, {"value": "0.0", "module": "B7", "scenario": "Standard scenario"}, {"value": "0.0", "module": "C1", "scenario": "Standard scenario"}, {"value": "0.0494", "module": "C2", "scenario": "Standard scenario"}, {"value": "2.06", "module": "C3", "scenario": "Standard scenario"}, {"value": "0.0156", "module": "C4", "scenario": "Standard scenario"}, {"value": "1.33", "module": "D", "scenario": "Standard scenario"}, {"name": "referenceToUnitGroupDataSet", "value": {"shortDescription": [{"value": "kg CO2-eq.", "lang": "en"}], "type": "unit group data set", "refObjectId": "1ebf3012-d0db-4de2-aefd-ef30cedb0be1", "version": "30.00.000", "uri": "../unitgroups/1ebf3012-d0db-4de2-aefd-ef30cedb0be1.xml"}}]}}, {"referenceToLCIAMethodDataSet": {"shortDescription": [{"value": "Global Warming Potential - land use and land use change (GWP-luluc)", "lang": "en"}, {"value": "Globales Erwärmungspotenzial - luluc (GWP-luluc)", "lang": "de"}], "type": "LCIA method data set", "refObjectId": "a7ea1ae2-9749-11ed-a8fc-0242ac120002", "version": "01.00.006", "uri": "../lciamethods/a7ea1ae2-9749-11ed-a8fc-0242ac120002.xml"}, "meanAmount": 0.0, "other": {"anies": [{"value": "0.162", "module": "A1", "scenario": "Standard scenario"}, {"value": "2.13E-4", "module": "A2", "scenario": "Standard scenario"}, {"value": "0.0039", "module": "A3", "scenario": "Standard scenario"}, {"value": "0.00123", "module": "A4", "scenario": "Standard scenario"}, {"value": "4.77E-5", "module": "A5", "scenario": "Standard scenario"}, {"value": "0.0", "module": "B1", "scenario": "Standard scenario"}, {"value": "0.0", "module": "B2", "scenario": "Standard scenario"}, {"value": "0.0", "module": "B3", "scenario": "Standard scenario"}, {"value": "0.0", "module": "B4", "scenario": "Standard scenario"}, {"value": "0.0", "module": "B5", "scenario": "Standard scenario"}, {"value": "0.655", "module": "B6", "scenario": "Standard scenario"}, {"value": "0.0", "module": "B7", "scenario": "Standard scenario"}, {"value": "0.0", "module": "C1", "scenario": "Standard scenario"}, {"value": "1.76E-4", "module": "C2", "scenario": "Standard scenario"}, {"value": "1.67E-4", "module": "C3", "scenario": "Standard scenario"}, {"value": "1.49E-6", "module": "C4", "scenario": "Standard scenario"}, {"value": "0.00665", "module": "D", "scenario": "Standard scenario"}, {"name": "referenceToUnitGroupDataSet", "value": {"shortDescription": [{"value": "kg CO2-eq.", "lang": "en"}], "type": "unit group data set", "refObjectId": "1ebf3012-d0db-4de2-aefd-ef30cedb0be1", "version": "30.00.000", "uri": "../unitgroups/1ebf3012-d0db-4de2-aefd-ef30cedb0be1.xml"}}]}}, {"referenceToLCIAMethodDataSet": {"shortDescription": [{"value": "Global Warming Potential - total (GWP-total)", "lang": "en"}, {"value": "Globales Erwärmungspotenzial - total (GWP-total)", "lang": "de"}], "type": "LCIA method data set", "refObjectId": "a7ea142a-9749-11ed-a8fc-0242ac120002", "version": "04.00.017", "uri": "../lciamethods/a7ea142a-9749-11ed-a8fc-0242ac120002.xml"}, "meanAmount": 0.0, "other": {"anies": [{"value": "94.3", "module": "A1", "scenario": "Standard scenario"}, {"value": "0.0598", "module": "A2", "scenario": "Standard scenario"}, {"value": "-0.624", "module": "A3", "scenario": "Standard scenario"}, {"value": "0.346", "module": "A4", "scenario": "Standard scenario"}, {"value": "1.29", "module": "A5", "scenario": "Standard scenario"}, {"value": "0.0", "module": "B1", "scenario": "Standard scenario"}, {"value": "0.0", "module": "B2", "scenario": "Standard scenario"}, {"value": "0.0", "module": "B3", "scenario": "Standard scenario"}, {"value": "0.0", "module": "B4", "scenario": "Standard scenario"}, {"value": "0.0", "module": "B5", "scenario": "Standard scenario"}, {"value": "264.0", "module": "B6", "scenario": "Standard scenario"}, {"value": "0.0", "module": "B7", "scenario": "Standard scenario"}, {"value": "0.0", "module": "C1", "scenario": "Standard scenario"}, {"value": "0.0496", "module": "C2", "scenario": "Standard scenario"}, {"value": "2.06", "module": "C3", "scenario": "Standard scenario"}, {"value": "0.0157", "module": "C4", "scenario": "Standard scenario"}, {"value": "1.35", "module": "D", "scenario": "Standard scenario"}, {"name": "referenceToUnitGroupDataSet", "value": {"shortDescription": [{"value": "kg CO2-eq.", "lang": "en"}], "type": "unit group data set", "refObjectId": "1ebf3012-d0db-4de2-aefd-ef30cedb0be1", "version": "30.00.000", "uri": "../unitgroups/1ebf3012-d0db-4de2-aefd-ef30cedb0be1.xml"}}]}}, {"referenceToLCIAMethodDataSet": {"shortDescription": [{"value": "Potential Comparative Toxic Unit for humans - cancer effects (HTP-c)", "lang": "en"}, {"value": "Potenzielle Toxizitätsvergleichseinheit für den Menschen - kanzerogene Wirkung (HTP-c)", "lang": "de"}], "type": "LCIA method data set", "refObjectId": "2299222a-bbd8-474f-9d4f-4dd1f18aea7c", "version": "01.00.004", "uri": "../lciamethods/2299222a-bbd8-474f-9d4f-4dd1f18aea7c.xml"}, "meanAmount": 0.0, "other": {"anies": [{"value": "2.2E-7", "module": "A1", "scenario": "Standard scenario"}, {"value": "3.16E-11", "module": "A2", "scenario": "Standard scenario"}, {"value": "7.8E-10", "module": "A3", "scenario": "Standard scenario"}, {"value": "1.82E-10", "module": "A4", "scenario": "Standard scenario"}, {"value": "9.74E-11", "module": "A5", "scenario": "Standard scenario"}, {"value": "0.0", "module": "B1", "scenario": "Standard scenario"}, {"value": "0.0", "module": "B2", "scenario": "Standard scenario"}, {"value": "0.0", "module": "B3", "scenario": "Standard scenario"}, {"value": "0.0", "module": "B4", "scenario": "Standard scenario"}, {"value": "0.0", "module": "B5", "scenario": "Standard scenario"}, {"value": "1.22E-7", "module": "B6", "scenario": "Standard scenario"}, {"value": "0.0", "module": "B7", "scenario": "Standard scenario"}, {"value": "0.0", "module": "C1", "scenario": "Standard scenario"}, {"value": "2.62E-11", "module": "C2", "scenario": "Standard scenario"}, {"value": "3.12E-10", "module": "C3", "scenario": "Standard scenario"}, {"value": "2.9E-12", "module": "C4", "scenario": "Standard scenario"}, {"value": "2.32E-8", "module": "D", "scenario": "Standard scenario"}, {"name": "referenceToUnitGroupDataSet", "value": {"shortDescription": [{"value": "CTUh", "lang": "en"}], "type": "unit group data set", "refObjectId": "d4c9523e-2d7e-49fd-8469-998f547d3a70", "version": "00.00.003", "uri": "../unitgroups/d4c9523e-2d7e-49fd-8469-998f547d3a70.xml"}}]}}, {"referenceToLCIAMethodDataSet": {"shortDescription": [{"value": "Potential Comparative Toxic Unit for humans - non-cancer effects (HTP-nc)", "lang": "en"}, {"value": "Potenzielle Toxizitätsvergleichseinheit für den Menschen - nicht kanzerogene Wirkung (HTP-nc)", "lang": "de"}], "type": "LCIA method data set", "refObjectId": "7cfdcfcf-b222-4b26-888a-a55f9fbf7ac8", "version": "01.00.003", "uri": "../lciamethods/7cfdcfcf-b222-4b26-888a-a55f9fbf7ac8.xml"}, "meanAmount": 0.0, "other": {"anies": [{"value": "5.05E-6", "module": "A1", "scenario": "Standard scenario"}, {"value": "6.86E-10", "module": "A2", "scenario": "Standard scenario"}, {"value": "3.24E-8", "module": "A3", "scenario": "Standard scenario"}, {"value": "3.96E-9", "module": "A4", "scenario": "Standard scenario"}, {"value": "7.05E-10", "module": "A5", "scenario": "Standard scenario"}, {"value": "0.0", "module": "B1", "scenario": "Standard scenario"}, {"value": "0.0", "module": "B2", "scenario": "Standard scenario"}, {"value": "0.0", "module": "B3", "scenario": "Standard scenario"}, {"value": "0.0", "module": "B4", "scenario": "Standard scenario"}, {"value": "0.0", "module": "B5", "scenario": "Standard scenario"}, {"value": "4.86E-6", "module": "B6", "scenario": "Standard scenario"}, {"value": "0.0", "module": "B7", "scenario": "Standard scenario"}, {"value": "0.0", "module": "C1", "scenario": "Standard scenario"}, {"value": "5.69E-10", "module": "C2", "scenario": "Standard scenario"}, {"value": "4.96E-8", "module": "C3", "scenario": "Standard scenario"}, {"value": "1.77E-10", "module": "C4", "scenario": "Standard scenario"}, {"value": "2.9E-7", "module": "D", "scenario": "Standard scenario"}, {"name": "referenceToUnitGroupDataSet", "value": {"shortDescription": [{"value": "CTUh", "lang": "en"}], "type": "unit group data set", "refObjectId": "d4c9523e-2d7e-49fd-8469-998f547d3a70", "version": "00.00.003", "uri": "../unitgroups/d4c9523e-2d7e-49fd-8469-998f547d3a70.xml"}}]}}, {"referenceToLCIAMethodDataSet": {"shortDescription": [{"value": "Potential Human exposure efficiency relative to U235 (IRP)", "lang": "en"}, {"value": "Potenzielle Wirkung durch Exposition des Menschen mit U235 (IRP)", "lang": "de"}], "type": "LCIA method data set", "refObjectId": "b5c632be-def3-11e6-bf01-fe55135034f3", "version": "01.00.012", "uri": "../lciamethods/b5c632be-def3-11e6-bf01-fe55135034f3.xml"}, "meanAmount": 0.0, "other": {"anies": [{"value": "21.9", "module": "A1", "scenario": "Standard scenario"}, {"value": "3.33E-4", "module": "A2", "scenario": "Standard scenario"}, {"value": "1.58", "module": "A3", "scenario": "Standard scenario"}, {"value": "0.00192", "module": "A4", "scenario": "Standard scenario"}, {"value": "7.0E-4", "module": "A5", "scenario": "Standard scenario"}, {"value": "0.0", "module": "B1", "scenario": "Standard scenario"}, {"value": "0.0", "module": "B2", "scenario": "Standard scenario"}, {"value": "0.0", "module": "B3", "scenario": "Standard scenario"}, {"value": "0.0", "module": "B4", "scenario": "Standard scenario"}, {"value": "0.0", "module": "B5", "scenario": "Standard scenario"}, {"value": "52.8", "module": "B6", "scenario": "Standard scenario"}, {"value": "0.0", "module": "B7", "scenario": "Standard scenario"}, {"value": "0.0", "module": "C1", "scenario": "Standard scenario"}, {"value": "2.76E-4", "module": "C2", "scenario": "Standard scenario"}, {"value": "0.00404", "module": "C3", "scenario": "Standard scenario"}, {"value": "6.66E-5", "module": "C4", "scenario": "Standard scenario"}, {"value": "0.222", "module": "D", "scenario": "Standard scenario"}, {"name": "referenceToUnitGroupDataSet", "value": {"shortDescription": [{"value": "kgBq U235-eq.", "lang": "en"}], "type": "unit group data set", "refObjectId": "456b05bf-1415-44a9-9993-02452f554c09", "version": "00.00.003", "uri": "../unitgroups/456b05bf-1415-44a9-9993-02452f554c09.xml"}}]}}, {"referenceToLCIAMethodDataSet": {"shortDescription": [{"value": "Depletion potential of the stratospheric ozone layer (ODP)", "lang": "en"}, {"value": "Abbaupotenzial der stratosphärischen Ozonschicht (ODP)", "lang": "de"}], "type": "LCIA method data set", "refObjectId": "b5c629d6-def3-11e6-bf01-fe55135034f3", "version": "02.00.013", "uri": "../lciamethods/b5c629d6-def3-11e6-bf01-fe55135034f3.xml"}, "meanAmount": 0.0, "other": {"anies": [{"value": "3.89E-6", "module": "A1", "scenario": "Standard scenario"}, {"value": "1.06E-9", "module": "A2", "scenario": "Standard scenario"}, {"value": "2.07E-8", "module": "A3", "scenario": "Standard scenario"}, {"value": "6.13E-9", "module": "A4", "scenario": "Standard scenario"}, {"value": "2.41E-9", "module": "A5", "scenario": "Standard scenario"}, {"value": "0.0", "module": "B1", "scenario": "Standard scenario"}, {"value": "0.0", "module": "B2", "scenario": "Standard scenario"}, {"value": "0.0", "module": "B3", "scenario": "Standard scenario"}, {"value": "0.0", "module": "B4", "scenario": "Standard scenario"}, {"value": "0.0", "module": "B5", "scenario": "Standard scenario"}, {"value": "4.99E-6", "module": "B6", "scenario": "Standard scenario"}, {"value": "0.0", "module": "B7", "scenario": "Standard scenario"}, {"value": "0.0", "module": "C1", "scenario": "Standard scenario"}, {"value": "8.79E-10", "module": "C2", "scenario": "Standard scenario"}, {"value": "2.5E-9", "module": "C3", "scenario": "Standard scenario"}, {"value": "7.7E-11", "module": "C4", "scenario": "Standard scenario"}, {"value": "-3.25E-8", "module": "D", "scenario": "Standard scenario"}, {"name": "referenceToUnitGroupDataSet", "value": {"shortDescription": [{"value": "kg CFC-11-eq.", "lang": "en"}], "type": "unit group data set", "refObjectId": "d9e957c9-7309-4474-bf3a-7777df6c4e5b", "version": "25.00.000", "uri": "../unitgroups/d9e957c9-7309-4474-bf3a-7777df6c4e5b.xml"}}]}}, {"referenceToLCIAMethodDataSet": {"shortDescription": [{"value": "Potential incidence of disease due to PM emissions (PM)", "lang": "en"}, {"value": "Potenzielles Auftreten von Krankheiten aufgrund von Feinstaubemissionen (PM)", "lang": "de"}], "type": "LCIA method data set", "refObjectId": "b5c602c6-def3-11e6-bf01-fe55135034f3", "version": "02.00.012", "uri": "../lciamethods/b5c602c6-def3-11e6-bf01-fe55135034f3.xml"}, "meanAmount": 0.0, "other": {"anies": [{"value": "5.34E-6", "module": "A1", "scenario": "Standard scenario"}, {"value": "5.89E-9", "module": "A2", "scenario": "Standard scenario"}, {"value": "7.25E-8", "module": "A3", "scenario": "Standard scenario"}, {"value": "3.4E-8", "module": "A4", "scenario": "Standard scenario"}, {"value": "4.95E-9", "module": "A5", "scenario": "Standard scenario"}, {"value": "0.0", "module": "B1", "scenario": "Standard scenario"}, {"value": "0.0", "module": "B2", "scenario": "Standard scenario"}, {"value": "0.0", "module": "B3", "scenario": "Standard scenario"}, {"value": "0.0", "module": "B4", "scenario": "Standard scenario"}, {"value": "0.0", "module": "B5", "scenario": "Standard scenario"}, {"value": "4.77E-6", "module": "B6", "scenario": "Standard scenario"}, {"value": "0.0", "module": "B7", "scenario": "Standard scenario"}, {"value": "0.0", "module": "C1", "scenario": "Standard scenario"}, {"value": "4.88E-9", "module": "C2", "scenario": "Standard scenario"}, {"value": "6.49E-9", "module": "C3", "scenario": "Standard scenario"}, {"value": "4.59E-10", "module": "C4", "scenario": "Standard scenario"}, {"value": "2.14E-9", "module": "D", "scenario": "Standard scenario"}, {"name": "referenceToUnitGroupDataSet", "value": {"shortDescription": [{"value": "Disease incidence", "lang": "en"}], "type": "unit group data set", "refObjectId": "3883559b-648f-4afc-8ba2-0bd24f3affa3", "version": "00.00.003", "uri": "../unitgroups/3883559b-648f-4afc-8ba2-0bd24f3affa3.xml"}}]}}, {"referenceToLCIAMethodDataSet": {"shortDescription": [{"value": "Photochemical Ozone Creation Potential (POCP)", "lang": "en"}, {"value": "Bildungspotenzial für troposphärisches Ozon (POCP)", "lang": "de"}], "type": "LCIA method data set", "refObjectId": "b5c610fe-def3-11e6-bf01-fe55135034f3", "version": "02.00.015", "uri": "../lciamethods/b5c610fe-def3-11e6-bf01-fe55135034f3.xml"}, "meanAmount": 0.0, "other": {"anies": [{"value": "0.43", "module": "A1", "scenario": "Standard scenario"}, {"value": "3.95E-4", "module": "A2", "scenario": "Standard scenario"}, {"value": "0.00379", "module": "A3", "scenario": "Standard scenario"}, {"value": "0.00228", "module": "A4", "scenario": "Standard scenario"}, {"value": "4.1E-4", "module": "A5", "scenario": "Standard scenario"}, {"value": "0.0", "module": "B1", "scenario": "Standard scenario"}, {"value": "0.0", "module": "B2", "scenario": "Standard scenario"}, {"value": "0.0", "module": "B3", "scenario": "Standard scenario"}, {"value": "0.0", "module": "B4", "scenario": "Standard scenario"}, {"value": "0.0", "module": "B5", "scenario": "Standard scenario"}, {"value": "0.705", "module": "B6", "scenario": "Standard scenario"}, {"value": "0.0", "module": "B7", "scenario": "Standard scenario"}, {"value": "0.0", "module": "C1", "scenario": "Standard scenario"}, {"value": "3.27E-4", "module": "C2", "scenario": "Standard scenario"}, {"value": "8.92E-4", "module": "C3", "scenario": "Standard scenario"}, {"value": "3.4E-5", "module": "C4", "scenario": "Standard scenario"}, {"value": "0.003", "module": "D", "scenario": "Standard scenario"}, {"name": "referenceToUnitGroupDataSet", "value": {"shortDescription": [{"value": "kg NMVOC-eq.", "lang": "en"}], "type": "unit group data set", "refObjectId": "d27c25f8-fbc1-44c6-b47b-4adbae4199c6", "version": "00.00.003", "uri": "../unitgroups/d27c25f8-fbc1-44c6-b47b-4adbae4199c6.xml"}}]}}, {"referenceToLCIAMethodDataSet": {"shortDescription": [{"value": "Potential Soil quality index (SQP)", "lang": "en"}, {"value": "Potenzieller Bodenqualitätsindex (SQP)", "lang": "de"}], "type": "LCIA method data set", "refObjectId": "b2ad6890-c78d-11e6-9d9d-cec0c932ce01", "version": "01.00.011", "uri": "../lciamethods/b2ad6890-c78d-11e6-9d9d-cec0c932ce01.xml"}, "meanAmount": 0.0, "other": {"anies": [{"value": "436.0", "module": "A1", "scenario": "Standard scenario"}, {"value": "0.674", "module": "A2", "scenario": "Standard scenario"}, {"value": "96.1", "module": "A3", "scenario": "Standard scenario"}, {"value": "3.89", "module": "A4", "scenario": "Standard scenario"}, {"value": "0.21", "module": "A5", "scenario": "Standard scenario"}, {"value": "0.0", "module": "B1", "scenario": "Standard scenario"}, {"value": "0.0", "module": "B2", "scenario": "Standard scenario"}, {"value": "0.0", "module": "B3", "scenario": "Standard scenario"}, {"value": "0.0", "module": "B4", "scenario": "Standard scenario"}, {"value": "0.0", "module": "B5", "scenario": "Standard scenario"}, {"value": "1160.0", "module": "B6", "scenario": "Standard scenario"}, {"value": "0.0", "module": "B7", "scenario": "Standard scenario"}, {"value": "0.0", "module": "C1", "scenario": "Standard scenario"}, {"value": "0.559", "module": "C2", "scenario": "Standard scenario"}, {"value": "0.474", "module": "C3", "scenario": "Standard scenario"}, {"value": "0.151", "module": "C4", "scenario": "Standard scenario"}, {"value": "-17.3", "module": "D", "scenario": "Standard scenario"}, {"name": "referenceToUnitGroupDataSet", "value": {"shortDescription": [{"value": "dimensionless", "lang": "en"}], "type": "unit group data set", "refObjectId": "f130951c-e67f-4f7f-8dd4-665de3974e18", "version": "00.00.004", "uri": "../unitgroups/f130951c-e67f-4f7f-8dd4-665de3974e18.xml"}}]}}, {"referenceToLCIAMethodDataSet": {"shortDescription": [{"value": "Water (user) deprivation potential (WDP)", "lang": "en"}, {"value": "Wasser-Entzugspotenzial (Benutzer) (WDP)", "lang": "de"}], "type": "LCIA method data set", "refObjectId": "b2ad66ce-c78d-11e6-9d9d-cec0c932ce01", "version": "03.00.015", "uri": "../lciamethods/b2ad66ce-c78d-11e6-9d9d-cec0c932ce01.xml"}, "meanAmount": 0.0, "other": {"anies": [{"value": "30.2", "module": "A1", "scenario": "Standard scenario"}, {"value": "0.00466", "module": "A2", "scenario": "Standard scenario"}, {"value": "0.339", "module": "A3", "scenario": "Standard scenario"}, {"value": "0.0269", "module": "A4", "scenario": "Standard scenario"}, {"value": "0.00636", "module": "A5", "scenario": "Standard scenario"}, {"value": "0.0", "module": "B1", "scenario": "Standard scenario"}, {"value": "0.0", "module": "B2", "scenario": "Standard scenario"}, {"value": "0.0", "module": "B3", "scenario": "Standard scenario"}, {"value": "0.0", "module": "B4", "scenario": "Standard scenario"}, {"value": "0.0", "module": "B5", "scenario": "Standard scenario"}, {"value": "66.9", "module": "B6", "scenario": "Standard scenario"}, {"value": "0.0", "module": "B7", "scenario": "Standard scenario"}, {"value": "0.0", "module": "C1", "scenario": "Standard scenario"}, {"value": "0.00386", "module": "C2", "scenario": "Standard scenario"}, {"value": "0.0473", "module": "C3", "scenario": "Standard scenario"}, {"value": "0.00146", "module": "C4", "scenario": "Standard scenario"}, {"value": "-1.64", "module": "D", "scenario": "Standard scenario"}, {"name": "referenceToUnitGroupDataSet", "value": {"shortDescription": [{"value": "m3 world eq. deprived", "lang": "en"}], "type": "unit group data set", "refObjectId": "6ae2df01-888e-46c8-b17d-49fa3869b476", "version": "00.00.003", "uri": "../unitgroups/6ae2df01-888e-46c8-b17d-49fa3869b476.xml"}}]}}]}, "otherAttributes": {"{http://www.indata.network/EPD/2019}epd-version": "1.2"}, "version": "1.1"}