{"processInformation": {"dataSetInformation": {"UUID": "36b263e1-0863-4c1c-a9fc-43210a39eec7", "name": {"baseName": [{"value": "Basic Sets", "lang": "en"}, {"value": "Grundkörper", "lang": "de"}], "functionalUnitFlowProperties": [{"lang": "en"}]}, "classificationInformation": {"classification": [{"class": [{"value": "Gebäudetechnik", "level": 0, "classId": "8"}, {"value": "Sanitär", "level": 1, "classId": "8.3"}, {"value": "Armaturen", "level": 2, "classId": "8.3.02"}], "name": "OEKOBAU.DAT"}, {"class": [{"value": "03 Building services engineering", "level": 0}, {"value": "Sanitary facilitys", "level": 1}, {"value": "Fittings and showers", "level": 2}], "name": "IBUCategories"}]}, "generalComment": [{"value": "Basic Sets essentially comprise of brass materials and several assembly parts of various materials.\n\n\nFor the use and application of the product the respective national provisions at the place of use apply, in Germany for example the building codes of the federal states and the corresponding national specifications.\n\nThe products comply with the applicable standards and regulations listed below.", "lang": "en"}]}, "quantitativeReference": {"referenceToReferenceFlow": [0]}, "time": {"referenceYear": 2023, "dataSetValidUntil": 2028, "other": {"anies": [{"name": "publicationDateOfEPD", "value": 1677196800000}]}}, "geography": {"locationOfOperationSupplyOrProduction": {"location": "GLO"}}, "technology": {"technologyDescriptionAndIncludedProcesses": [{"value": "No. 1: The sand core for the base body is made. No. 2: The body is cast from brass using the sand core. No. 3: After casting, the brass body is grinded. No. 4: The plastic parts of the body are injected. No. 5: The product parts are assembled. No. 6: The preassembled product is packed together with the remaining components (like enclosed pack). Any production waste generated is disposed accordingly. In individual cases, the production may differ slightly from the procedure (for example, if the brass body is purchased and not manufactured in-house). \nDeclared unit: \nThe results of this EPD are valid for the following functional unit:\n\nProvide sanitary function for one (1) average basic set unit used in accordance with the manufacturer's recommendations for a 20-year life, following the manufacturer's operating instructions. An average conditioned basic set is considered the baseline flow. \n\n Weighted averaging based on production tonnages in 2020 is chosen as basis for creating the environmental profile. 80 different basic sets were considered.", "lang": "en"}, {"value": "Nr. 1: Der Sandkern für den Grundkörper wird hergestellt. \n\nNr. 2: Der Körper wird aus Messing unter Verwendung des Sandkerns gegossen. \n\nNr. 3: Nach dem Gießen wird der Messingkörper geschliffen. \n\nNr. 4: Die Kunststoffteile des Körpers werden gespritzt. \n\nNr. 5: Die Produktteile werden zusammengesetzt. \n\nNr. 6: Das vormontierte Produkt wird zusammen mit den übrigen Komponenten verpackt (wie eine beiliegende Packung). \n\nAnfallende Produktionsabfälle werden entsprechend entsorgt. In Einzelfällen kann die Produktion geringfügig von diesem Verfahren abweichen (z. B. wenn der Messingkörper zugekauft und nicht selbst hergestellt wird). \n", "lang": "de"}], "technologicalApplicability": [{"value": "Basic Sets are plumbing fixtures that direct water to the end-user products. They are located concealed in the wall and need further products (end-user products) to work. The products are used in bathrooms and rest rooms. Examples for end-user products are thermostats, overhead showers or shower faucets.", "lang": "en"}, {"value": "Basic Sets sind Sanitärarmaturen, die das Wasser zu den Endverbraucherprodukten leiten. Sie befinden sich verdeckt in der Wand und benötigen weitere Produkte (Endverbraucherprodukte), um zu funktionieren. Die Produkte werden in Badezimmern und Ruheräumen verwendet. Beispiele für Endverbraucherprodukte sind Thermostate, Kopfbrausen oder Duscharmaturen.", "lang": "de"}]}}, "modellingAndValidation": {"LCIMethodAndAllocation": {"typeOfDataSet": "EPD", "referenceToLCAMethodDetails": [{"shortDescription": [{"value": "Fittings and showers.pdf", "lang": "en"}], "type": "source data set", "refObjectId": "64f8db9b-5aaa-46d8-add2-9f6a50cd07d2"}], "other": {"anies": [{"name": "subType", "value": "average dataset"}]}}, "dataSourcesTreatmentAndRepresentativeness": {"referenceToDataSource": [{"shortDescription": [{"value": "GaBi Database (all versions)", "lang": "en"}], "type": "source data set", "refObjectId": "28d74cc0-db8b-4d7e-bc44-5f6d56ce0c4a"}, {"shortDescription": [{"value": "GaBi Database Edition 2021, CUP 2021.02", "lang": "en"}], "type": "source data set", "refObjectId": "90321ffe-9ebb-4946-886c-338efe6fbf26"}], "useAdviceForDataSet": [{"value": "Scope: \nThis average EPD was determined on the basis of a weighted average of production volume from 2020 and relates to the plants in Wasselonne, France, Offenburg and Schiltach, Germany and Alpharetta, USA. This average EPD is valid for the whole product group basic sets. The EPD was formed from >98% of the products involved in the sales quantity. \nSystem boundary: \nThis representative EPD follows the EPD type \"cradle to gate - with options\". The following life cycle modules are declared:\n\n Modules A1-A3:  \n\n The product stage begins with considering the production of the necessary raw materials and energies, including all corresponding upstream chains and the actual procurement transports. Furthermore, the entire manufacturing phase was mapped, including the treatment of production waste until the end-of-waste status (EoW) was reached. Green electricity from hydropower is used for the manufacturing processes in Germany. Green electricity from hydropower and wind power (50% each) is used for the French production site. US electricity mix is used for the US production site. \n\n Module A4: \n\n All distribution transports to the customers were considered. \n\n Module A5: \n\n This module covers the installation process with the corresponding packaging waste generated that needs to be disposed. \n\nModule B1-B7:\n\nThese modules were considered, but evaluated as not relevant for the products and considered as zero.Modules C1-C4: \n\n The modules include the environmental impacts for dismantling of the products and the treatment of the waste fractions until the end-of-waste status (EoW) is reached, including the associated transports at the end of the product life cycle. \n\n Module D: \n\nIdentification of the benefits and costs of the product outside the system boundary. For waste, paper and plastics, these consist of energy credits from thermal utilization (A3, A5 and C3) in the form of the average European electricity mix or thermal energy from natural gas. Recycling of paper, plastic and metal scrap results in credits of the respective raw materials for the primary material portion of the input. The loads of the waste incineration and recycling processes are assigned to the respective modules (A3, A5 and C3) and not to module D.", "lang": "en"}], "other": {"anies": [{"name": "referenceToOriginalEPD", "value": {"shortDescription": {"value": "Basic Sets.pdf", "defaultValue": "Basic Sets.pdf", "lstrings": [{"lang": "en", "value": "Basic Sets.pdf"}]}, "type": "source data set", "uuid": {"uuid": "8e8db8bf-9724-4854-b165-da95f8416aa2"}, "refObjectId": "8e8db8bf-9724-4854-b165-da95f8416aa2", "resourceURLs": ["https://oekobaudat.de/OEKOBAU.DAT/resource/sources/8e8db8bf-9724-4854-b165-da95f8416aa2/Basic_Sets_14890.pdf?version=00.01.000"]}}]}}, "validation": {"review": [{"referenceToNameOfReviewerAndInstitution": [{"shortDescription": [{"value": "Institut Bauen und Umwelt e. V.", "lang": "en"}], "type": "contact data set", "refObjectId": "d111dbec-b024-4be5-86c5-752d6eb2cf95", "uri": "../contacts/d111dbec-b024-4be5-86c5-752d6eb2cf95.xml"}], "type": "Accredited third party review"}]}, "complianceDeclarations": {"compliance": [{"referenceToComplianceSystem": {"shortDescription": [{"value": "DIN EN 15804+A2", "lang": "en"}], "type": "source data set", "refObjectId": "c0016b33-8cf7-415c-ac6e-deba0d21440d", "uri": "../sources/c0016b33-8cf7-415c-ac6e-deba0d21440d.xml"}}, {"referenceToComplianceSystem": {"shortDescription": [{"value": "ISO 14025", "lang": "en"}], "type": "source data set", "refObjectId": "4f2eb655-6e44-4874-a95a-e28f5442cd4d", "uri": "../sources/4f2eb655-6e44-4874-a95a-e28f5442cd4d.xml"}}]}}, "administrativeInformation": {"commissionerAndGoal": {"referenceToCommissioner": [{"shortDescription": [{"value": "Hansgrohe Group", "lang": "en"}], "type": "contact data set", "refObjectId": "e2e7bc1a-4fae-4c47-9754-a0a4995bdebe", "uri": "../contacts/e2e7bc1a-4fae-4c47-9754-a0a4995bdebe.xml"}]}, "dataGenerator": {"referenceToPersonOrEntityGeneratingTheDataSet": [{"shortDescription": [{"value": "brands and values GmbH", "lang": "en"}], "type": "contact data set", "refObjectId": "6b539b8a-10e3-4004-8ccc-a79f169aa339", "uri": "../contacts/6b539b8a-10e3-4004-8ccc-a79f169aa339.xml"}]}, "dataEntryBy": {"timeStamp": 1677238000252, "referenceToDataSetFormat": [{"shortDescription": [{"value": "ILCD Format", "lang": "en"}], "type": "source data set", "refObjectId": "a97a0155-0234-4b87-b4ce-a45da52f2a40", "uri": "../sources/a97a0155-0234-4b87-b4ce-a45da52f2a40.xml"}, {"shortDescription": [{"value": "EPD-Datenformaterweiterungen v1.2", "lang": "de"}, {"value": "EPD Data Format Extensions v1.2", "lang": "en"}], "type": "source data set", "refObjectId": "a29449fd-aa2f-4de8-b5d7-4b06b43c6fde", "uri": "../sources/a29449fd-aa2f-4de8-b5d7-4b06b43c6fde.xml"}]}, "publicationAndOwnership": {"dataSetVersion": "00.01.000", "referenceToRegistrationAuthority": {"shortDescription": [{"value": "Institut Bauen und Umwelt e. V.", "lang": "en"}], "type": "contact data set", "refObjectId": "d111dbec-b024-4be5-86c5-752d6eb2cf95", "uri": "../contacts/d111dbec-b024-4be5-86c5-752d6eb2cf95.xml"}, "registrationNumber": "EPD-HAN-20230025-ICC1-EN", "referenceToOwnershipOfDataSet": {"shortDescription": [{"value": "Hansgrohe Group", "lang": "en"}], "type": "contact data set", "refObjectId": "e2e7bc1a-4fae-4c47-9754-a0a4995bdebe", "uri": "../contacts/e2e7bc1a-4fae-4c47-9754-a0a4995bdebe.xml"}, "copyright": true, "licenseType": "Free of charge for all users and uses", "accessRestrictions": [{"value": "None", "lang": "en"}], "other": {"anies": [{"name": "referenceToPublisher", "value": {"shortDescription": [{"value": "Institut Bauen und Umwelt e. V.", "lang": "en"}], "type": "contact data set", "refObjectId": "d111dbec-b024-4be5-86c5-752d6eb2cf95", "uri": "../contacts/d111dbec-b024-4be5-86c5-752d6eb2cf95.xml"}}]}}}, "exchanges": {"exchange": [{"dataSetInternalID": 0, "referenceToFlowDataSet": {"shortDescription": [{"value": "Basic set ()", "lang": "en"}], "type": "flow data set", "refObjectId": "929c524d-c7ac-d304-1e6b-ea957ac68439", "uri": "../flows/929c524d-c7ac-d304-1e6b-ea957ac68439.xml"}, "meanAmount": 1.0, "referencesToDataSource": {}, "referenceFlow": true, "resolvedFlowVersion": "00.01.000", "resultingflowAmount": 1.0, "flowProperties": [{"name": [{"lang": "en", "value": "Number of pieces"}, {"lang": "de", "value": "Anzahl"}], "uuid": "01846770-4cfe-4a25-8ad9-919d8d378345", "referenceFlowProperty": true, "meanValue": 1.0, "referenceUnit": "pcs.", "unitGroupUUID": "934110e3-baf4-49e9-992c-3d8109a6aafb"}], "materialProperties": [{"name": "mass reference", "value": "1.417", "unit": "kg/m^3", "unitDescription": "Kilogram per cubic meter "}], "typeOfFlow": "Product flow", "classification": {"classHierarchy": "Gebäudetechnik / Sanitär / Armaturen", "name": "OEKOBAU.DAT"}}, {"dataSetInternalID": 1, "referenceToFlowDataSet": {"shortDescription": [{"value": "Renewable primary energy as energy carrier (PERE)", "lang": "en"}, {"value": "Erneuerbare Primärenergie als Energieträger (PERE)", "lang": "de"}], "type": "flow data set", "refObjectId": "20f32be5-0398-4288-9b6d-accddd195317", "uri": "../flows/20f32be5-0398-4288-9b6d-accddd195317.xml"}, "exchange direction": "INPUT", "other": {"anies": [{"name": "referenceToUnitGroupDataSet", "value": {"shortDescription": [{"value": "MJ", "lang": "en"}], "type": "unit group data set", "refObjectId": "93a60a57-a3c8-11da-a746-0800200c9a66", "uri": "../unitgroups/93a60a57-a3c8-11da-a746-0800200c9a66.xml"}}, {"value": "6.32839097501301", "module": "A1-A3"}, {"value": "0.0601", "module": "A4"}, {"value": "5.31160902498699", "module": "A5"}, {"value": "0", "module": "B1"}, {"value": "0", "module": "B2"}, {"value": "0", "module": "B3"}, {"value": "0", "module": "B4"}, {"value": "0", "module": "B5"}, {"value": "0", "module": "B6"}, {"value": "0", "module": "B7"}, {"value": "0", "module": "C1"}, {"value": "0.0153", "module": "C2"}, {"value": "0.189", "module": "C3"}, {"value": "0.00333", "module": "C4"}, {"value": "-1.76", "module": "D"}]}, "resolvedFlowVersion": "38.00.000", "flowProperties": [], "typeOfFlow": "Other flow", "classification": {"classHierarchy": "Quantities", "name": "GaBiCategories"}}, {"dataSetInternalID": 2, "referenceToFlowDataSet": {"shortDescription": [{"value": "Renewable primary energy resources as material utilization (PERM)", "lang": "en"}, {"value": "Erneuerbare Primärenergie zur stofflichen Nutzung (PERM)", "lang": "de"}], "type": "flow data set", "refObjectId": "fb3ec0de-548d-4508-aea5-00b73bf6f702", "uri": "../flows/fb3ec0de-548d-4508-aea5-00b73bf6f702.xml"}, "exchange direction": "INPUT", "other": {"anies": [{"name": "referenceToUnitGroupDataSet", "value": {"shortDescription": [{"value": "MJ", "lang": "en"}], "type": "unit group data set", "refObjectId": "93a60a57-a3c8-11da-a746-0800200c9a66", "uri": "../unitgroups/93a60a57-a3c8-11da-a746-0800200c9a66.xml"}}, {"value": "3.97160902498699", "module": "A1-A3"}, {"value": "0", "module": "A4"}, {"value": "-3.97160902498699", "module": "A5"}, {"value": "0", "module": "B1"}, {"value": "0", "module": "B2"}, {"value": "0", "module": "B3"}, {"value": "0", "module": "B4"}, {"value": "0", "module": "B5"}, {"value": "0", "module": "B6"}, {"value": "0", "module": "B7"}, {"value": "0", "module": "C1"}, {"value": "0", "module": "C2"}, {"value": "0", "module": "C3"}, {"value": "0", "module": "C4"}, {"value": "0", "module": "D"}]}, "resolvedFlowVersion": "38.00.000", "flowProperties": [], "typeOfFlow": "Other flow", "classification": {"classHierarchy": "Quantities", "name": "GaBiCategories"}}, {"dataSetInternalID": 3, "referenceToFlowDataSet": {"shortDescription": [{"value": "Total use of renewable primary energy resources (PERT)", "lang": "en"}, {"value": "Total erneuerbare Primärenergie (PERT)", "lang": "de"}], "type": "flow data set", "refObjectId": "53f97275-fa8a-4cdd-9024-65936002acd0", "uri": "../flows/53f97275-fa8a-4cdd-9024-65936002acd0.xml"}, "exchange direction": "INPUT", "other": {"anies": [{"name": "referenceToUnitGroupDataSet", "value": {"shortDescription": [{"value": "MJ", "lang": "en"}], "type": "unit group data set", "refObjectId": "93a60a57-a3c8-11da-a746-0800200c9a66", "uri": "../unitgroups/93a60a57-a3c8-11da-a746-0800200c9a66.xml"}}, {"value": "10.3", "module": "A1-A3"}, {"value": "0.0601", "module": "A4"}, {"value": "1.34", "module": "A5"}, {"value": "0", "module": "B1"}, {"value": "0", "module": "B2"}, {"value": "0", "module": "B3"}, {"value": "0", "module": "B4"}, {"value": "0", "module": "B5"}, {"value": "0", "module": "B6"}, {"value": "0", "module": "B7"}, {"value": "0", "module": "C1"}, {"value": "0.0153", "module": "C2"}, {"value": "0.189", "module": "C3"}, {"value": "0.00333", "module": "C4"}, {"value": "-1.76", "module": "D"}]}, "resolvedFlowVersion": "38.00.000", "flowProperties": [], "typeOfFlow": "Other flow", "classification": {"classHierarchy": "Quantities / Environmental quantities / EPD EN 15804 / LCI indicators", "name": "GaBiCategories"}}, {"dataSetInternalID": 4, "referenceToFlowDataSet": {"shortDescription": [{"value": "Non renewable primary energy as energy carrier (PENRE)", "lang": "en"}, {"value": "Nicht-erneuerbare Primärenergie als Energieträger (PENRE)", "lang": "de"}], "type": "flow data set", "refObjectId": "ac857178-2b45-46ec-892a-a9a4332f0372", "uri": "../flows/ac857178-2b45-46ec-892a-a9a4332f0372.xml"}, "exchange direction": "INPUT", "other": {"anies": [{"name": "referenceToUnitGroupDataSet", "value": {"shortDescription": [{"value": "MJ", "lang": "en"}], "type": "unit group data set", "refObjectId": "93a60a57-a3c8-11da-a746-0800200c9a66", "uri": "../unitgroups/93a60a57-a3c8-11da-a746-0800200c9a66.xml"}}, {"value": "36.158103046345", "module": "A1-A3"}, {"value": "1.67", "module": "A4"}, {"value": "4.69627118486203", "module": "A5"}, {"value": "0", "module": "B1"}, {"value": "0", "module": "B2"}, {"value": "0", "module": "B3"}, {"value": "0", "module": "B4"}, {"value": "0", "module": "B5"}, {"value": "0", "module": "B6"}, {"value": "0", "module": "B7"}, {"value": "0", "module": "C1"}, {"value": "0.266", "module": "C2"}, {"value": "10.1313444803533", "module": "C3"}, {"value": "0.0459", "module": "C4"}, {"value": "-4.64", "module": "D"}]}, "resolvedFlowVersion": "38.00.000", "flowProperties": [], "typeOfFlow": "Other flow", "classification": {"classHierarchy": "Quantities", "name": "GaBiCategories"}}, {"dataSetInternalID": 5, "referenceToFlowDataSet": {"shortDescription": [{"value": "Non renewable primary energy as material utilization (PENRM)", "lang": "en"}, {"value": "Nicht-erneuerbare Primärenergie zur stofflichen Nutzung (PENRM)", "lang": "de"}], "type": "flow data set", "refObjectId": "1421caa0-679d-4bf4-b282-0eb850ccae27", "uri": "../flows/1421caa0-679d-4bf4-b282-0eb850ccae27.xml"}, "exchange direction": "INPUT", "other": {"anies": [{"name": "referenceToUnitGroupDataSet", "value": {"shortDescription": [{"value": "MJ", "lang": "en"}], "type": "unit group data set", "refObjectId": "93a60a57-a3c8-11da-a746-0800200c9a66", "uri": "../unitgroups/93a60a57-a3c8-11da-a746-0800200c9a66.xml"}}, {"value": "10.341896953655", "module": "A1-A3"}, {"value": "0", "module": "A4"}, {"value": "-0.156271184862033", "module": "A5"}, {"value": "0", "module": "B1"}, {"value": "0", "module": "B2"}, {"value": "0", "module": "B3"}, {"value": "0", "module": "B4"}, {"value": "0", "module": "B5"}, {"value": "0", "module": "B6"}, {"value": "0", "module": "B7"}, {"value": "0", "module": "C1"}, {"value": "0", "module": "C2"}, {"value": "-9.67634448035328", "module": "C3"}, {"value": "0", "module": "C4"}, {"value": "0", "module": "D"}]}, "resolvedFlowVersion": "38.00.000", "flowProperties": [], "typeOfFlow": "Other flow", "classification": {"classHierarchy": "Quantities", "name": "GaBiCategories"}}, {"dataSetInternalID": 6, "referenceToFlowDataSet": {"shortDescription": [{"value": "Total use of non renewable primary energy resources (PENRT)", "lang": "en"}, {"value": "Total nicht erneuerbare Primärenergie (PENRT)", "lang": "de"}], "type": "flow data set", "refObjectId": "06159210-646b-4c8d-8583-da9b3b95a6c1", "uri": "../flows/06159210-646b-4c8d-8583-da9b3b95a6c1.xml"}, "exchange direction": "INPUT", "other": {"anies": [{"name": "referenceToUnitGroupDataSet", "value": {"shortDescription": [{"value": "MJ", "lang": "en"}], "type": "unit group data set", "refObjectId": "93a60a57-a3c8-11da-a746-0800200c9a66", "uri": "../unitgroups/93a60a57-a3c8-11da-a746-0800200c9a66.xml"}}, {"value": "46.5", "module": "A1-A3"}, {"value": "1.67", "module": "A4"}, {"value": "4.54", "module": "A5"}, {"value": "0", "module": "B1"}, {"value": "0", "module": "B2"}, {"value": "0", "module": "B3"}, {"value": "0", "module": "B4"}, {"value": "0", "module": "B5"}, {"value": "0", "module": "B6"}, {"value": "0", "module": "B7"}, {"value": "0", "module": "C1"}, {"value": "0.266", "module": "C2"}, {"value": "0.455", "module": "C3"}, {"value": "0.0459", "module": "C4"}, {"value": "-4.64", "module": "D"}]}, "resolvedFlowVersion": "38.00.000", "flowProperties": [], "typeOfFlow": "Other flow", "classification": {"classHierarchy": "Quantities / Environmental quantities / EPD EN 15804 / LCI indicators", "name": "GaBiCategories"}}, {"dataSetInternalID": 7, "referenceToFlowDataSet": {"shortDescription": [{"value": "Use of secondary material (SM)", "lang": "en"}, {"value": "Einsatz von Sekundärstoffen (SM)", "lang": "de"}], "type": "flow data set", "refObjectId": "c6a1f35f-2d09-4f54-8dfb-97e502e1ce92", "uri": "../flows/c6a1f35f-2d09-4f54-8dfb-97e502e1ce92.xml"}, "exchange direction": "INPUT", "other": {"anies": [{"name": "referenceToUnitGroupDataSet", "value": {"shortDescription": [{"value": "kg", "lang": "en"}], "type": "unit group data set", "refObjectId": "ad38d542-3fe9-439d-9b95-2f5f7752acaf", "uri": "../unitgroups/ad38d542-3fe9-439d-9b95-2f5f7752acaf.xml"}}, {"value": "1.05", "module": "A1-A3"}, {"value": "0", "module": "A4"}, {"value": "0", "module": "A5"}, {"value": "0", "module": "B1"}, {"value": "0", "module": "B2"}, {"value": "0", "module": "B3"}, {"value": "0", "module": "B4"}, {"value": "0", "module": "B5"}, {"value": "0", "module": "B6"}, {"value": "0", "module": "B7"}, {"value": "0", "module": "C1"}, {"value": "0", "module": "C2"}, {"value": "0", "module": "C3"}, {"value": "0", "module": "C4"}, {"value": "0.128", "module": "D"}]}, "resolvedFlowVersion": "38.00.000", "flowProperties": [], "typeOfFlow": "Other flow", "classification": {"classHierarchy": "Quantities / Environmental quantities / EPD EN 15804 / LCI indicators", "name": "GaBiCategories"}}, {"dataSetInternalID": 8, "referenceToFlowDataSet": {"shortDescription": [{"value": "Use of renewable secondary fuels (RSF)", "lang": "en"}, {"value": "Erneuerbare Sekundärbrennstoffe (RSF)", "lang": "de"}], "type": "flow data set", "refObjectId": "64333088-a55f-4aa2-9a31-c10b07816787", "uri": "../flows/64333088-a55f-4aa2-9a31-c10b07816787.xml"}, "exchange direction": "INPUT", "other": {"anies": [{"name": "referenceToUnitGroupDataSet", "value": {"shortDescription": [{"value": "MJ", "lang": "en"}], "type": "unit group data set", "refObjectId": "93a60a57-a3c8-11da-a746-0800200c9a66", "uri": "../unitgroups/93a60a57-a3c8-11da-a746-0800200c9a66.xml"}}, {"value": "0", "module": "A1-A3"}, {"value": "0", "module": "A4"}, {"value": "0", "module": "A5"}, {"value": "0", "module": "B1"}, {"value": "0", "module": "B2"}, {"value": "0", "module": "B3"}, {"value": "0", "module": "B4"}, {"value": "0", "module": "B5"}, {"value": "0", "module": "B6"}, {"value": "0", "module": "B7"}, {"value": "0", "module": "C1"}, {"value": "0", "module": "C2"}, {"value": "0", "module": "C3"}, {"value": "0", "module": "C4"}, {"value": "0", "module": "D"}]}, "resolvedFlowVersion": "38.00.000", "flowProperties": [], "typeOfFlow": "Other flow", "classification": {"classHierarchy": "Quantities / Environmental quantities / EPD EN 15804 / LCI indicators", "name": "GaBiCategories"}}, {"dataSetInternalID": 9, "referenceToFlowDataSet": {"shortDescription": [{"value": "Use of non renewable secondary fuels (NRSF)", "lang": "en"}, {"value": "Nicht erneuerbare Sekundärbrennstoffe (NRSF)", "lang": "de"}], "type": "flow data set", "refObjectId": "89def144-d39a-4287-b86f-efde453ddcb2", "uri": "../flows/89def144-d39a-4287-b86f-efde453ddcb2.xml"}, "exchange direction": "INPUT", "other": {"anies": [{"name": "referenceToUnitGroupDataSet", "value": {"shortDescription": [{"value": "MJ", "lang": "en"}], "type": "unit group data set", "refObjectId": "93a60a57-a3c8-11da-a746-0800200c9a66", "uri": "../unitgroups/93a60a57-a3c8-11da-a746-0800200c9a66.xml"}}, {"value": "0", "module": "A1-A3"}, {"value": "0", "module": "A4"}, {"value": "0", "module": "A5"}, {"value": "0", "module": "B1"}, {"value": "0", "module": "B2"}, {"value": "0", "module": "B3"}, {"value": "0", "module": "B4"}, {"value": "0", "module": "B5"}, {"value": "0", "module": "B6"}, {"value": "0", "module": "B7"}, {"value": "0", "module": "C1"}, {"value": "0", "module": "C2"}, {"value": "0", "module": "C3"}, {"value": "0", "module": "C4"}, {"value": "0", "module": "D"}]}, "resolvedFlowVersion": "38.00.000", "flowProperties": [], "typeOfFlow": "Other flow", "classification": {"classHierarchy": "Quantities / Environmental quantities / EPD EN 15804 / LCI indicators", "name": "GaBiCategories"}}, {"dataSetInternalID": 10, "referenceToFlowDataSet": {"shortDescription": [{"value": "Use of net fresh water (FW)", "lang": "en"}, {"value": "Einsatz von Süßwasserressourcen (FW)", "lang": "de"}], "type": "flow data set", "refObjectId": "3cf952c8-f3a4-461d-8c96-96456ca62246", "uri": "../flows/3cf952c8-f3a4-461d-8c96-96456ca62246.xml"}, "exchange direction": "INPUT", "other": {"anies": [{"name": "referenceToUnitGroupDataSet", "value": {"shortDescription": [{"value": "m^3", "lang": "en"}], "type": "unit group data set", "refObjectId": "cd950537-0a98-4044-9ba7-9f9a68d0a504", "uri": "../unitgroups/cd950537-0a98-4044-9ba7-9f9a68d0a504.xml"}}, {"value": "0.0332", "module": "A1-A3"}, {"value": "6.99E-05", "module": "A4"}, {"value": "0.00228", "module": "A5"}, {"value": "0", "module": "B1"}, {"value": "0", "module": "B2"}, {"value": "0", "module": "B3"}, {"value": "0", "module": "B4"}, {"value": "0", "module": "B5"}, {"value": "0", "module": "B6"}, {"value": "0", "module": "B7"}, {"value": "0", "module": "C1"}, {"value": "1.75E-05", "module": "C2"}, {"value": "0.00169", "module": "C3"}, {"value": "5.12E-07", "module": "C4"}, {"value": "-0.0179", "module": "D"}]}, "resolvedFlowVersion": "38.00.000", "flowProperties": [], "typeOfFlow": "Other flow", "classification": {"classHierarchy": "Quantities / Environmental quantities / EPD EN 15804 / LCI indicators", "name": "GaBiCategories"}}, {"dataSetInternalID": 11, "referenceToFlowDataSet": {"shortDescription": [{"value": "Hazardous waste disposed (HWD)", "lang": "en"}, {"value": "Gefährlicher Abfall zur Deponie (HWD)", "lang": "de"}], "type": "flow data set", "refObjectId": "430f9e0f-59b2-46a0-8e0d-55e0e84948fc", "uri": "../flows/430f9e0f-59b2-46a0-8e0d-55e0e84948fc.xml"}, "exchange direction": "OUTPUT", "other": {"anies": [{"name": "referenceToUnitGroupDataSet", "value": {"shortDescription": [{"value": "kg", "lang": "en"}], "type": "unit group data set", "refObjectId": "ad38d542-3fe9-439d-9b95-2f5f7752acaf", "uri": "../unitgroups/ad38d542-3fe9-439d-9b95-2f5f7752acaf.xml"}}, {"value": "6.69E-06", "module": "A1-A3"}, {"value": "5.83E-11", "module": "A4"}, {"value": "2.6E-09", "module": "A5"}, {"value": "0", "module": "B1"}, {"value": "0", "module": "B2"}, {"value": "0", "module": "B3"}, {"value": "0", "module": "B4"}, {"value": "0", "module": "B5"}, {"value": "0", "module": "B6"}, {"value": "0", "module": "B7"}, {"value": "0", "module": "C1"}, {"value": "1.4E-11", "module": "C2"}, {"value": "1.29E-10", "module": "C3"}, {"value": "8.16E-12", "module": "C4"}, {"value": "-7.23E-06", "module": "D"}]}, "resolvedFlowVersion": "38.00.000", "flowProperties": [], "typeOfFlow": "Other flow", "classification": {"classHierarchy": "Quantities / Environmental quantities / EPD EN 15804 / LCI indicators", "name": "GaBiCategories"}}, {"dataSetInternalID": 12, "referenceToFlowDataSet": {"shortDescription": [{"value": "Non hazardous waste disposed (NHWD)", "lang": "en"}, {"value": "Entsorgter nicht gefährlicher Abfall (NHWD)", "lang": "de"}], "type": "flow data set", "refObjectId": "b29ef66b-e286-4afa-949f-62f1a7b4d7fa", "uri": "../flows/b29ef66b-e286-4afa-949f-62f1a7b4d7fa.xml"}, "exchange direction": "OUTPUT", "other": {"anies": [{"name": "referenceToUnitGroupDataSet", "value": {"shortDescription": [{"value": "kg", "lang": "en"}], "type": "unit group data set", "refObjectId": "ad38d542-3fe9-439d-9b95-2f5f7752acaf", "uri": "../unitgroups/ad38d542-3fe9-439d-9b95-2f5f7752acaf.xml"}}, {"value": "0.237", "module": "A1-A3"}, {"value": "0.000224", "module": "A4"}, {"value": "0.0428", "module": "A5"}, {"value": "0", "module": "B1"}, {"value": "0", "module": "B2"}, {"value": "0", "module": "B3"}, {"value": "0", "module": "B4"}, {"value": "0", "module": "B5"}, {"value": "0", "module": "B6"}, {"value": "0", "module": "B7"}, {"value": "0", "module": "C1"}, {"value": "4.17E-05", "module": "C2"}, {"value": "0.0272", "module": "C3"}, {"value": "0.0587", "module": "C4"}, {"value": "-0.0818", "module": "D"}]}, "resolvedFlowVersion": "38.00.000", "flowProperties": [], "typeOfFlow": "Other flow", "classification": {"classHierarchy": "Quantities / Environmental quantities / EPD EN 15804 / LCI indicators", "name": "GaBiCategories"}}, {"dataSetInternalID": 13, "referenceToFlowDataSet": {"shortDescription": [{"value": "Radioactive waste disposed (RWD)", "lang": "en"}, {"value": "Entsorgter radioaktiver Abfall (RWD)", "lang": "de"}], "type": "flow data set", "refObjectId": "3449546e-52ad-4b39-b809-9fb77cea8ff6", "uri": "../flows/3449546e-52ad-4b39-b809-9fb77cea8ff6.xml"}, "exchange direction": "OUTPUT", "other": {"anies": [{"name": "referenceToUnitGroupDataSet", "value": {"shortDescription": [{"value": "kg", "lang": "en"}], "type": "unit group data set", "refObjectId": "ad38d542-3fe9-439d-9b95-2f5f7752acaf", "uri": "../unitgroups/ad38d542-3fe9-439d-9b95-2f5f7752acaf.xml"}}, {"value": "0.00102", "module": "A1-A3"}, {"value": "2.56E-06", "module": "A4"}, {"value": "0.000154", "module": "A5"}, {"value": "0", "module": "B1"}, {"value": "0", "module": "B2"}, {"value": "0", "module": "B3"}, {"value": "0", "module": "B4"}, {"value": "0", "module": "B5"}, {"value": "0", "module": "B6"}, {"value": "0", "module": "B7"}, {"value": "0", "module": "C1"}, {"value": "4.83E-07", "module": "C2"}, {"value": "2.75E-05", "module": "C3"}, {"value": "5.26E-07", "module": "C4"}, {"value": "-0.0001", "module": "D"}]}, "resolvedFlowVersion": "38.00.000", "flowProperties": [], "typeOfFlow": "Other flow", "classification": {"classHierarchy": "Quantities / Environmental quantities / EPD EN 15804 / LCI indicators", "name": "GaBiCategories"}}, {"dataSetInternalID": 14, "referenceToFlowDataSet": {"shortDescription": [{"value": "Components for re-use (CRU)", "lang": "en"}, {"value": "Komponenten für die Wiederverwendung (CRU)", "lang": "de"}], "type": "flow data set", "refObjectId": "a2b32f97-3fc7-4af2-b209-525bc6426f33", "uri": "../flows/a2b32f97-3fc7-4af2-b209-525bc6426f33.xml"}, "exchange direction": "OUTPUT", "other": {"anies": [{"name": "referenceToUnitGroupDataSet", "value": {"shortDescription": [{"value": "kg", "lang": "en"}], "type": "unit group data set", "refObjectId": "ad38d542-3fe9-439d-9b95-2f5f7752acaf", "uri": "../unitgroups/ad38d542-3fe9-439d-9b95-2f5f7752acaf.xml"}}, {"value": "0", "module": "A1-A3"}, {"value": "0", "module": "A4"}, {"value": "0", "module": "A5"}, {"value": "0", "module": "B1"}, {"value": "0", "module": "B2"}, {"value": "0", "module": "B3"}, {"value": "0", "module": "B4"}, {"value": "0", "module": "B5"}, {"value": "0", "module": "B6"}, {"value": "0", "module": "B7"}, {"value": "0", "module": "C1"}, {"value": "0", "module": "C2"}, {"value": "0", "module": "C3"}, {"value": "0", "module": "C4"}, {"value": "0", "module": "D"}]}, "resolvedFlowVersion": "38.00.000", "flowProperties": [], "typeOfFlow": "Other flow", "classification": {"classHierarchy": "Quantities / Environmental quantities / EPD EN 15804 / LCI indicators", "name": "GaBiCategories"}}, {"dataSetInternalID": 15, "referenceToFlowDataSet": {"shortDescription": [{"value": "Materials for recycling (MFR)", "lang": "en"}, {"value": "Stoffe zum Recycling (MFR)", "lang": "de"}], "type": "flow data set", "refObjectId": "d7fe48a5-4103-49c8-9aae-b0b5dfdbd6ae", "uri": "../flows/d7fe48a5-4103-49c8-9aae-b0b5dfdbd6ae.xml"}, "exchange direction": "OUTPUT", "other": {"anies": [{"name": "referenceToUnitGroupDataSet", "value": {"shortDescription": [{"value": "kg", "lang": "en"}], "type": "unit group data set", "refObjectId": "ad38d542-3fe9-439d-9b95-2f5f7752acaf", "uri": "../unitgroups/ad38d542-3fe9-439d-9b95-2f5f7752acaf.xml"}}, {"value": "0", "module": "A1-A3"}, {"value": "0", "module": "A4"}, {"value": "0.219", "module": "A5"}, {"value": "0", "module": "B1"}, {"value": "0", "module": "B2"}, {"value": "0", "module": "B3"}, {"value": "0", "module": "B4"}, {"value": "0", "module": "B5"}, {"value": "0", "module": "B6"}, {"value": "0", "module": "B7"}, {"value": "0", "module": "C1"}, {"value": "0", "module": "C2"}, {"value": "0.803", "module": "C3"}, {"value": "0", "module": "C4"}, {"value": "0", "module": "D"}]}, "resolvedFlowVersion": "38.00.000", "flowProperties": [], "typeOfFlow": "Other flow", "classification": {"classHierarchy": "Quantities / Environmental quantities / EPD EN 15804 / LCI indicators", "name": "GaBiCategories"}}, {"dataSetInternalID": 16, "referenceToFlowDataSet": {"shortDescription": [{"value": "Materials for energy recovery (MER)", "lang": "en"}, {"value": "Stoffe für die Energierückgewinnung (MER)", "lang": "de"}], "type": "flow data set", "refObjectId": "59a9181c-3aaf-46ee-8b13-2b3723b6e447", "uri": "../flows/59a9181c-3aaf-46ee-8b13-2b3723b6e447.xml"}, "exchange direction": "OUTPUT", "other": {"anies": [{"name": "referenceToUnitGroupDataSet", "value": {"shortDescription": [{"value": "kg", "lang": "en"}], "type": "unit group data set", "refObjectId": "ad38d542-3fe9-439d-9b95-2f5f7752acaf", "uri": "../unitgroups/ad38d542-3fe9-439d-9b95-2f5f7752acaf.xml"}}, {"value": "0", "module": "A1-A3"}, {"value": "0", "module": "A4"}, {"value": "0", "module": "A5"}, {"value": "0", "module": "B1"}, {"value": "0", "module": "B2"}, {"value": "0", "module": "B3"}, {"value": "0", "module": "B4"}, {"value": "0", "module": "B5"}, {"value": "0", "module": "B6"}, {"value": "0", "module": "B7"}, {"value": "0", "module": "C1"}, {"value": "0", "module": "C2"}, {"value": "0", "module": "C3"}, {"value": "0", "module": "C4"}, {"value": "0", "module": "D"}]}, "resolvedFlowVersion": "38.00.000", "flowProperties": [], "typeOfFlow": "Other flow", "classification": {"classHierarchy": "Quantities / Environmental quantities / EPD EN 15804 / LCI indicators", "name": "GaBiCategories"}}, {"dataSetInternalID": 17, "referenceToFlowDataSet": {"shortDescription": [{"value": "Exported electrical energy (EEE)", "lang": "en"}, {"value": "Exportierte elektrische Energie (EEE)", "lang": "de"}], "type": "flow data set", "refObjectId": "4da0c987-2b76-40d6-9e9e-82a017aaaf29", "uri": "../flows/4da0c987-2b76-40d6-9e9e-82a017aaaf29.xml"}, "exchange direction": "OUTPUT", "other": {"anies": [{"name": "referenceToUnitGroupDataSet", "value": {"shortDescription": [{"value": "MJ", "lang": "en"}], "type": "unit group data set", "refObjectId": "93a60a57-a3c8-11da-a746-0800200c9a66", "uri": "../unitgroups/93a60a57-a3c8-11da-a746-0800200c9a66.xml"}}, {"value": "0.016", "module": "A1-A3"}, {"value": "0", "module": "A4"}, {"value": "0.0578", "module": "A5"}, {"value": "0", "module": "B1"}, {"value": "0", "module": "B2"}, {"value": "0", "module": "B3"}, {"value": "0", "module": "B4"}, {"value": "0", "module": "B5"}, {"value": "0", "module": "B6"}, {"value": "0", "module": "B7"}, {"value": "0", "module": "C1"}, {"value": "0", "module": "C2"}, {"value": "0.00873", "module": "C3"}, {"value": "8.76E-05", "module": "C4"}, {"value": "0", "module": "D"}]}, "resolvedFlowVersion": "38.00.000", "flowProperties": [], "typeOfFlow": "Other flow", "classification": {"classHierarchy": "Quantities / Environmental quantities / EPD EN 15804 / LCI indicators", "name": "GaBiCategories"}}, {"dataSetInternalID": 18, "referenceToFlowDataSet": {"shortDescription": [{"value": "Exported thermal energy (EET)", "lang": "en"}, {"value": "Exportierte thermische Energie (EET)", "lang": "de"}], "type": "flow data set", "refObjectId": "98daf38a-7a79-46d3-9a37-2b7bd0955810", "uri": "../flows/98daf38a-7a79-46d3-9a37-2b7bd0955810.xml"}, "exchange direction": "OUTPUT", "other": {"anies": [{"name": "referenceToUnitGroupDataSet", "value": {"shortDescription": [{"value": "MJ", "lang": "en"}], "type": "unit group data set", "refObjectId": "93a60a57-a3c8-11da-a746-0800200c9a66", "uri": "../unitgroups/93a60a57-a3c8-11da-a746-0800200c9a66.xml"}}, {"value": "0.0317", "module": "A1-A3"}, {"value": "0", "module": "A4"}, {"value": "0.104", "module": "A5"}, {"value": "0", "module": "B1"}, {"value": "0", "module": "B2"}, {"value": "0", "module": "B3"}, {"value": "0", "module": "B4"}, {"value": "0", "module": "B5"}, {"value": "0", "module": "B6"}, {"value": "0", "module": "B7"}, {"value": "0", "module": "C1"}, {"value": "0", "module": "C2"}, {"value": "0.0164", "module": "C3"}, {"value": "0", "module": "C4"}, {"value": "0", "module": "D"}]}, "resolvedFlowVersion": "38.00.000", "flowProperties": [], "typeOfFlow": "Other flow", "classification": {"classHierarchy": "Quantities / Environmental quantities / EPD EN 15804 / LCI indicators", "name": "GaBiCategories"}}]}, "LCIAResults": {"LCIAResult": [{"referenceToLCIAMethodDataSet": {"shortDescription": [{"value": "Global Warming Potential total (GWP-total)", "lang": "en"}, {"value": "Globales Erwärmungspotenzial total (GWP-total)", "lang": "de"}], "type": "LCIA method data set", "refObjectId": "6a37f984-a4b3-458a-a20a-64418c145fa2", "uri": "../lciamethods/6a37f984-a4b3-458a-a20a-64418c145fa2.xml"}, "other": {"anies": [{"name": "referenceToUnitGroupDataSet", "value": {"shortDescription": [{"value": "kg CO_(2)-Äq.", "lang": "en"}], "type": "unit group data set", "refObjectId": "1ebf3012-d0db-4de2-aefd-ef30cedb0be1", "uri": "../unitgroups/1ebf3012-d0db-4de2-aefd-ef30cedb0be1.xml"}}, {"value": "2.20213", "module": "A1-A3"}, {"value": "0.130618", "module": "A4"}, {"value": "0.624343", "module": "A5"}, {"value": "0", "module": "B1"}, {"value": "0", "module": "B2"}, {"value": "0", "module": "B3"}, {"value": "0", "module": "B4"}, {"value": "0", "module": "B5"}, {"value": "0", "module": "B6"}, {"value": "0", "module": "B7"}, {"value": "0", "module": "C1"}, {"value": "0.019963", "module": "C2"}, {"value": "0.6110602", "module": "C3"}, {"value": "0.00317302", "module": "C4"}, {"value": "-0.748413506480151", "module": "D"}]}}, {"referenceToLCIAMethodDataSet": {"shortDescription": [{"value": "Global Warming Potential fossil fuels (GWP-fossil)", "lang": "en"}, {"value": "Globales Erwärmungspotenzial fossil (GWP-fossil)", "lang": "de"}], "type": "LCIA method data set", "refObjectId": "5f635281-343e-44fb-83df-1971b155e6b6", "uri": "../lciamethods/5f635281-343e-44fb-83df-1971b155e6b6.xml"}, "other": {"anies": [{"name": "referenceToUnitGroupDataSet", "value": {"shortDescription": [{"value": "kg CO_(2)-Äq.", "lang": "en"}], "type": "unit group data set", "refObjectId": "1ebf3012-d0db-4de2-aefd-ef30cedb0be1", "uri": "../unitgroups/1ebf3012-d0db-4de2-aefd-ef30cedb0be1.xml"}}, {"value": "2.55", "module": "A1-A3"}, {"value": "0.13", "module": "A4"}, {"value": "0.27", "module": "A5"}, {"value": "0", "module": "B1"}, {"value": "0", "module": "B2"}, {"value": "0", "module": "B3"}, {"value": "0", "module": "B4"}, {"value": "0", "module": "B5"}, {"value": "0", "module": "B6"}, {"value": "0", "module": "B7"}, {"value": "0", "module": "C1"}, {"value": "0.0198", "module": "C2"}, {"value": "0.611", "module": "C3"}, {"value": "0.00317", "module": "C4"}, {"value": "-0.398", "module": "D"}]}}, {"referenceToLCIAMethodDataSet": {"shortDescription": [{"value": "Global Warming Potential biogenic (GWP-biogenic)", "lang": "en"}, {"value": "Globales Erwärmungspotenzial biogen (GWP-biogenic)", "lang": "de"}], "type": "LCIA method data set", "refObjectId": "2356e1ab-0185-4db5-86e5-16de51c7485c", "uri": "../lciamethods/2356e1ab-0185-4db5-86e5-16de51c7485c.xml"}, "other": {"anies": [{"name": "referenceToUnitGroupDataSet", "value": {"shortDescription": [{"value": "kg CO_(2)-Äq.", "lang": "en"}], "type": "unit group data set", "refObjectId": "1ebf3012-d0db-4de2-aefd-ef30cedb0be1", "uri": "../unitgroups/1ebf3012-d0db-4de2-aefd-ef30cedb0be1.xml"}}, {"value": "-0.354", "module": "A1-A3"}, {"value": "0", "module": "A4"}, {"value": "0.354", "module": "A5"}, {"value": "0", "module": "B1"}, {"value": "0", "module": "B2"}, {"value": "0", "module": "B3"}, {"value": "0", "module": "B4"}, {"value": "0", "module": "B5"}, {"value": "0", "module": "B6"}, {"value": "0", "module": "B7"}, {"value": "0", "module": "C1"}, {"value": "0", "module": "C2"}, {"value": "0", "module": "C3"}, {"value": "0", "module": "C4"}, {"value": "-0.349133506480151", "module": "D"}]}}, {"referenceToLCIAMethodDataSet": {"shortDescription": [{"value": "Global Warming Potential luluc (GWP-luluc)", "lang": "en"}, {"value": "Globales Erwärmungspotenzial luluc (GWP-luluc)", "lang": "de"}], "type": "LCIA method data set", "refObjectId": "4331bbdb-978a-490d-8707-eeb047f01a55", "uri": "../lciamethods/4331bbdb-978a-490d-8707-eeb047f01a55.xml"}, "other": {"anies": [{"name": "referenceToUnitGroupDataSet", "value": {"shortDescription": [{"value": "kg CO_(2)-Äq.", "lang": "en"}], "type": "unit group data set", "refObjectId": "1ebf3012-d0db-4de2-aefd-ef30cedb0be1", "uri": "../unitgroups/1ebf3012-d0db-4de2-aefd-ef30cedb0be1.xml"}}, {"value": "0.00613", "module": "A1-A3"}, {"value": "0.000618", "module": "A4"}, {"value": "0.000343", "module": "A5"}, {"value": "0", "module": "B1"}, {"value": "0", "module": "B2"}, {"value": "0", "module": "B3"}, {"value": "0", "module": "B4"}, {"value": "0", "module": "B5"}, {"value": "0", "module": "B6"}, {"value": "0", "module": "B7"}, {"value": "0", "module": "C1"}, {"value": "0.000163", "module": "C2"}, {"value": "6.02E-05", "module": "C3"}, {"value": "3.02E-06", "module": "C4"}, {"value": "-0.00128", "module": "D"}]}}, {"referenceToLCIAMethodDataSet": {"shortDescription": [{"value": "Depletion potential of the stratospheric ozone layer (ODP)", "lang": "en"}, {"value": "Abbau Potential der stratosphärischen Ozonschicht (ODP)", "lang": "de"}], "type": "LCIA method data set", "refObjectId": "b5c629d6-def3-11e6-bf01-fe55135034f3", "uri": "../lciamethods/b5c629d6-def3-11e6-bf01-fe55135034f3.xml"}, "other": {"anies": [{"name": "referenceToUnitGroupDataSet", "value": {"shortDescription": [{"value": "kg CFC11-Äq.", "lang": "en"}], "type": "unit group data set", "refObjectId": "d9e957c9-7309-4474-bf3a-7777df6c4e5b", "uri": "../unitgroups/d9e957c9-7309-4474-bf3a-7777df6c4e5b.xml"}}, {"value": "6.01E-09", "module": "A1-A3"}, {"value": "2.05E-17", "module": "A4"}, {"value": "1.97E-15", "module": "A5"}, {"value": "0", "module": "B1"}, {"value": "0", "module": "B2"}, {"value": "0", "module": "B3"}, {"value": "0", "module": "B4"}, {"value": "0", "module": "B5"}, {"value": "0", "module": "B6"}, {"value": "0", "module": "B7"}, {"value": "0", "module": "C1"}, {"value": "3.93E-18", "module": "C2"}, {"value": "6.93E-11", "module": "C3"}, {"value": "7.51E-18", "module": "C4"}, {"value": "-6.07E-09", "module": "D"}]}}, {"referenceToLCIAMethodDataSet": {"shortDescription": [{"value": "Acidification potential of land and water (AP)", "lang": "en"}, {"value": "Versauerungspotenzial von Boden und Wasser (AP)", "lang": "de"}], "type": "LCIA method data set", "refObjectId": "b5c611c6-def3-11e6-bf01-fe55135034f3", "uri": "../lciamethods/b5c611c6-def3-11e6-bf01-fe55135034f3.xml"}, "other": {"anies": [{"name": "referenceToUnitGroupDataSet", "value": {"shortDescription": [{"value": "mol H^(+)-Äq.", "lang": "en"}], "type": "unit group data set", "refObjectId": "42e089ac-92bf-4bf2-8ca1-5fc40d18f2ed", "uri": "../unitgroups/42e089ac-92bf-4bf2-8ca1-5fc40d18f2ed.xml"}}, {"value": "0.0161", "module": "A1-A3"}, {"value": "0.00213", "module": "A4"}, {"value": "0.00102", "module": "A5"}, {"value": "0", "module": "B1"}, {"value": "0", "module": "B2"}, {"value": "0", "module": "B3"}, {"value": "0", "module": "B4"}, {"value": "0", "module": "B5"}, {"value": "0", "module": "B6"}, {"value": "0", "module": "B7"}, {"value": "0", "module": "C1"}, {"value": "3.33E-05", "module": "C2"}, {"value": "0.000382", "module": "C3"}, {"value": "9.93E-06", "module": "C4"}, {"value": "-0.0048", "module": "D"}]}}, {"referenceToLCIAMethodDataSet": {"shortDescription": [{"value": "Eutrophication potential aquatic freshwater (EP-freshwater)", "lang": "en"}, {"value": "Eutrophierungspotenzial Süßwasser (EP-freshwater)", "lang": "de"}], "type": "LCIA method data set", "refObjectId": "b53ec18f-7377-4ad3-86eb-cc3f4f276b2b", "uri": "../lciamethods/b53ec18f-7377-4ad3-86eb-cc3f4f276b2b.xml"}, "other": {"anies": [{"name": "referenceToUnitGroupDataSet", "value": {"shortDescription": [{"value": "kg PO_(4)-Äq.", "lang": "en"}], "type": "unit group data set", "refObjectId": "0429039d-a61d-4590-ba67-aa4a20a810a1", "uri": "../unitgroups/0429039d-a61d-4590-ba67-aa4a20a810a1.xml"}}, {"value": "0.000186", "module": "A1-A3"}, {"value": "2.36E-07", "module": "A4"}, {"value": "4.23E-07", "module": "A5"}, {"value": "0", "module": "B1"}, {"value": "0", "module": "B2"}, {"value": "0", "module": "B3"}, {"value": "0", "module": "B4"}, {"value": "0", "module": "B5"}, {"value": "0", "module": "B6"}, {"value": "0", "module": "B7"}, {"value": "0", "module": "C1"}, {"value": "5.91E-08", "module": "C2"}, {"value": "1E-07", "module": "C3"}, {"value": "1.84E-07", "module": "C4"}, {"value": "-0.000156", "module": "D"}]}}, {"referenceToLCIAMethodDataSet": {"shortDescription": [{"value": "Eutrophication potential aquatic marine (EP-marine)", "lang": "en"}, {"value": "Eutrophierungspotenzial Salzwasser (EP-marine)", "lang": "de"}], "type": "LCIA method data set", "refObjectId": "b5c619fa-def3-11e6-bf01-fe55135034f3", "uri": "../lciamethods/b5c619fa-def3-11e6-bf01-fe55135034f3.xml"}, "other": {"anies": [{"name": "referenceToUnitGroupDataSet", "value": {"shortDescription": [{"value": "kg N-Äq.", "lang": "en"}], "type": "unit group data set", "refObjectId": "d05bb823-ecdf-4686-8c40-bf1d9257859f", "uri": "../unitgroups/d05bb823-ecdf-4686-8c40-bf1d9257859f.xml"}}, {"value": "0.00239", "module": "A1-A3"}, {"value": "0.000578", "module": "A4"}, {"value": "0.000179", "module": "A5"}, {"value": "0", "module": "B1"}, {"value": "0", "module": "B2"}, {"value": "0", "module": "B3"}, {"value": "0", "module": "B4"}, {"value": "0", "module": "B5"}, {"value": "0", "module": "B6"}, {"value": "0", "module": "B7"}, {"value": "0", "module": "C1"}, {"value": "1.31E-05", "module": "C2"}, {"value": "0.000176", "module": "C3"}, {"value": "2.45E-06", "module": "C4"}, {"value": "-0.00064", "module": "D"}]}}, {"referenceToLCIAMethodDataSet": {"shortDescription": [{"value": "Eutrophication potential terrestrial (EP-terrestrial)", "lang": "en"}, {"value": "Eutrophierungspotenzial Land (EP-terrestrial)", "lang": "de"}], "type": "LCIA method data set", "refObjectId": "b5c614d2-def3-11e6-bf01-fe55135034f3", "uri": "../lciamethods/b5c614d2-def3-11e6-bf01-fe55135034f3.xml"}, "other": {"anies": [{"name": "referenceToUnitGroupDataSet", "value": {"shortDescription": [{"value": "mol N-Äq.", "lang": "en"}], "type": "unit group data set", "refObjectId": "71b4d617-0ec9-4d3f-b65e-e438940c2401", "uri": "../unitgroups/71b4d617-0ec9-4d3f-b65e-e438940c2401.xml"}}, {"value": "0.0253", "module": "A1-A3"}, {"value": "0.00636", "module": "A4"}, {"value": "0.00196", "module": "A5"}, {"value": "0", "module": "B1"}, {"value": "0", "module": "B2"}, {"value": "0", "module": "B3"}, {"value": "0", "module": "B4"}, {"value": "0", "module": "B5"}, {"value": "0", "module": "B6"}, {"value": "0", "module": "B7"}, {"value": "0", "module": "C1"}, {"value": "0.00015", "module": "C2"}, {"value": "0.00203", "module": "C3"}, {"value": "2.65E-05", "module": "C4"}, {"value": "-0.0071", "module": "D"}]}}, {"referenceToLCIAMethodDataSet": {"shortDescription": [{"value": "Formation potential of tropospheric ozone photochemical oxidants (POCP)", "lang": "en"}, {"value": "Bildungspotential für troposphärisches Ozon (POCP)", "lang": "de"}], "type": "LCIA method data set", "refObjectId": "b5c610fe-def3-11e6-bf01-fe55135034f3", "uri": "../lciamethods/b5c610fe-def3-11e6-bf01-fe55135034f3.xml"}, "other": {"anies": [{"name": "referenceToUnitGroupDataSet", "value": {"shortDescription": [{"value": "kg NMVOC-Äq.", "lang": "en"}], "type": "unit group data set", "refObjectId": "d27c25f8-fbc1-44c6-b47b-4adbae4199c6", "uri": "../unitgroups/d27c25f8-fbc1-44c6-b47b-4adbae4199c6.xml"}}, {"value": "0.00707", "module": "A1-A3"}, {"value": "0.00159", "module": "A4"}, {"value": "0.0006", "module": "A5"}, {"value": "0", "module": "B1"}, {"value": "0", "module": "B2"}, {"value": "0", "module": "B3"}, {"value": "0", "module": "B4"}, {"value": "0", "module": "B5"}, {"value": "0", "module": "B6"}, {"value": "0", "module": "B7"}, {"value": "0", "module": "C1"}, {"value": "2.97E-05", "module": "C2"}, {"value": "0.000453", "module": "C3"}, {"value": "7.71E-06", "module": "C4"}, {"value": "-0.00189", "module": "D"}]}}, {"referenceToLCIAMethodDataSet": {"shortDescription": [{"value": "Abiotic depletion potential for non fossil resources (ADPE)", "lang": "en"}, {"value": "Potenzial für den abiotischen Abbau nicht fossiler Ressourcen (ADPE)", "lang": "de"}], "type": "LCIA method data set", "refObjectId": "b2ad6494-c78d-11e6-9d9d-cec0c932ce01", "uri": "../lciamethods/b2ad6494-c78d-11e6-9d9d-cec0c932ce01.xml"}, "other": {"anies": [{"name": "referenceToUnitGroupDataSet", "value": {"shortDescription": [{"value": "kg Sb-Äq.", "lang": "en"}], "type": "unit group data set", "refObjectId": "54ccd2d9-a32a-4fc2-923d-f2c8c93e89d4", "uri": "../unitgroups/54ccd2d9-a32a-4fc2-923d-f2c8c93e89d4.xml"}}, {"value": "0.000715", "module": "A1-A3"}, {"value": "8.32E-09", "module": "A4"}, {"value": "5.69E-06", "module": "A5"}, {"value": "0", "module": "B1"}, {"value": "0", "module": "B2"}, {"value": "0", "module": "B3"}, {"value": "0", "module": "B4"}, {"value": "0", "module": "B5"}, {"value": "0", "module": "B6"}, {"value": "0", "module": "B7"}, {"value": "0", "module": "C1"}, {"value": "1.76E-09", "module": "C2"}, {"value": "9.6E-09", "module": "C3"}, {"value": "2.18E-10", "module": "C4"}, {"value": "-0.000343", "module": "D"}]}}, {"referenceToLCIAMethodDataSet": {"shortDescription": [{"value": "Abiotic depletion potential for fossil resources (ADPF)", "lang": "en"}, {"value": "Potenzial für den abiotischen Abbau fossiler Brennstoffe (ADPF)", "lang": "de"}], "type": "LCIA method data set", "refObjectId": "b2ad6110-c78d-11e6-9d9d-cec0c932ce01", "uri": "../lciamethods/b2ad6110-c78d-11e6-9d9d-cec0c932ce01.xml"}, "other": {"anies": [{"name": "referenceToUnitGroupDataSet", "value": {"shortDescription": [{"value": "MJ", "lang": "en"}], "type": "unit group data set", "refObjectId": "93a60a57-a3c8-11da-a746-0800200c9a66", "uri": "../unitgroups/93a60a57-a3c8-11da-a746-0800200c9a66.xml"}}, {"value": "46.5", "module": "A1-A3"}, {"value": "1.66", "module": "A4"}, {"value": "4.54", "module": "A5"}, {"value": "0", "module": "B1"}, {"value": "0", "module": "B2"}, {"value": "0", "module": "B3"}, {"value": "0", "module": "B4"}, {"value": "0", "module": "B5"}, {"value": "0", "module": "B6"}, {"value": "0", "module": "B7"}, {"value": "0", "module": "C1"}, {"value": "0.265", "module": "C2"}, {"value": "0.455", "module": "C3"}, {"value": "0.0459", "module": "C4"}, {"value": "-4.64", "module": "D"}]}}, {"referenceToLCIAMethodDataSet": {"shortDescription": [{"value": "Water use (WDP)", "lang": "en"}, {"value": "Wassernutzung (WDP)", "lang": "de"}], "type": "LCIA method data set", "refObjectId": "b2ad66ce-c78d-11e6-9d9d-cec0c932ce01", "uri": "../lciamethods/b2ad66ce-c78d-11e6-9d9d-cec0c932ce01.xml"}, "other": {"anies": [{"name": "referenceToUnitGroupDataSet", "value": {"shortDescription": [{"value": "m^(3) world-Äq. deprived", "lang": "en"}], "type": "unit group data set", "refObjectId": "6ae2df01-888e-46c8-b17d-49fa3869b476", "uri": "../unitgroups/6ae2df01-888e-46c8-b17d-49fa3869b476.xml"}}, {"value": "1.27", "module": "A1-A3"}, {"value": "0.000783", "module": "A4"}, {"value": "0.0659", "module": "A5"}, {"value": "0", "module": "B1"}, {"value": "0", "module": "B2"}, {"value": "0", "module": "B3"}, {"value": "0", "module": "B4"}, {"value": "0", "module": "B5"}, {"value": "0", "module": "B6"}, {"value": "0", "module": "B7"}, {"value": "0", "module": "C1"}, {"value": "0.000185", "module": "C2"}, {"value": "0.0691", "module": "C3"}, {"value": "-3.57E-05", "module": "C4"}, {"value": "-0.777", "module": "D"}]}}, {"referenceToLCIAMethodDataSet": {"shortDescription": [{"value": "Incidence of disease due to PM emissions (PM)", "lang": "en"}, {"value": "Auftreten von Krankheiten aufgrund von Feinstaubemissionen (PM)", "lang": "de"}], "type": "LCIA method data set", "refObjectId": "b5c602c6-def3-11e6-bf01-fe55135034f3", "uri": "../lciamethods/b5c602c6-def3-11e6-bf01-fe55135034f3.xml"}, "other": {"anies": [{"name": "referenceToUnitGroupDataSet", "value": {"shortDescription": [{"value": "Disease incidence", "lang": "en"}], "type": "unit group data set", "refObjectId": "3883559b-648f-4afc-8ba2-0bd24f3affa3", "uri": "../unitgroups/3883559b-648f-4afc-8ba2-0bd24f3affa3.xml"}}, {"value": "1.41E-07", "module": "A1-A3"}, {"value": "3.5E-08", "module": "A4"}, {"value": "1.45E-08", "module": "A5"}, {"value": "0", "module": "B1"}, {"value": "0", "module": "B2"}, {"value": "0", "module": "B3"}, {"value": "0", "module": "B4"}, {"value": "0", "module": "B5"}, {"value": "0", "module": "B6"}, {"value": "0", "module": "B7"}, {"value": "0", "module": "C1"}, {"value": "2.08E-10", "module": "C2"}, {"value": "1.7E-09", "module": "C3"}, {"value": "1.05E-10", "module": "C4"}, {"value": "-4.8E-08", "module": "D"}]}}, {"referenceToLCIAMethodDataSet": {"shortDescription": [{"value": "Human exposure efficiency relative to U235 (IR)", "lang": "en"}, {"value": "Wirkung durch Exposition des Menschen mit U235 (IR)", "lang": "de"}], "type": "LCIA method data set", "refObjectId": "b5c632be-def3-11e6-bf01-fe55135034f3", "uri": "../lciamethods/b5c632be-def3-11e6-bf01-fe55135034f3.xml"}, "other": {"anies": [{"name": "referenceToUnitGroupDataSet", "value": {"shortDescription": [{"value": "kBq U235-Äq.", "lang": "en"}], "type": "unit group data set", "refObjectId": "456b05bf-1415-44a9-9993-02452f554c09", "uri": "../unitgroups/456b05bf-1415-44a9-9993-02452f554c09.xml"}}, {"value": "0.174", "module": "A1-A3"}, {"value": "0.000372", "module": "A4"}, {"value": "0.0233", "module": "A5"}, {"value": "0", "module": "B1"}, {"value": "0", "module": "B2"}, {"value": "0", "module": "B3"}, {"value": "0", "module": "B4"}, {"value": "0", "module": "B5"}, {"value": "0", "module": "B6"}, {"value": "0", "module": "B7"}, {"value": "0", "module": "C1"}, {"value": "7.06E-05", "module": "C2"}, {"value": "0.00283", "module": "C3"}, {"value": "7.54E-05", "module": "C4"}, {"value": "-0.0319", "module": "D"}]}}, {"referenceToLCIAMethodDataSet": {"shortDescription": [{"value": "Comparative toxic unit for ecosystems (ETP-fw)", "lang": "en"}, {"value": "Toxizitätsvergleichseinheit für Ökosysteme (ETP-fw)", "lang": "de"}], "type": "LCIA method data set", "refObjectId": "ee1082d1-b0f7-43ca-a1f0-21e2a4a74511", "uri": "../lciamethods/ee1082d1-b0f7-43ca-a1f0-21e2a4a74511.xml"}, "other": {"anies": [{"name": "referenceToUnitGroupDataSet", "value": {"shortDescription": [{"value": "CTUe", "lang": "en"}], "type": "unit group data set", "refObjectId": "aa959ded-f1eb-4efb-9c5c-2d60be36b3e6", "uri": "../unitgroups/aa959ded-f1eb-4efb-9c5c-2d60be36b3e6.xml"}}, {"value": "72.1", "module": "A1-A3"}, {"value": "1.22", "module": "A4"}, {"value": "1.73", "module": "A5"}, {"value": "0", "module": "B1"}, {"value": "0", "module": "B2"}, {"value": "0", "module": "B3"}, {"value": "0", "module": "B4"}, {"value": "0", "module": "B5"}, {"value": "0", "module": "B6"}, {"value": "0", "module": "B7"}, {"value": "0", "module": "C1"}, {"value": "0.197", "module": "C2"}, {"value": "0.275", "module": "C3"}, {"value": "0.0229", "module": "C4"}, {"value": "-25.1", "module": "D"}]}}, {"referenceToLCIAMethodDataSet": {"shortDescription": [{"value": "Comparative toxic unit for humans (carcinogenic) (HTP-c)", "lang": "en"}, {"value": "Toxizitätsvergleichseinheit für Menschen (krebserregend) (HTP-c)", "lang": "de"}], "type": "LCIA method data set", "refObjectId": "2299222a-bbd8-474f-9d4f-4dd1f18aea7c", "uri": "../lciamethods/2299222a-bbd8-474f-9d4f-4dd1f18aea7c.xml"}, "other": {"anies": [{"name": "referenceToUnitGroupDataSet", "value": {"shortDescription": [{"value": "CTUh", "lang": "en"}], "type": "unit group data set", "refObjectId": "d4c9523e-2d7e-49fd-8469-998f547d3a70", "uri": "../unitgroups/d4c9523e-2d7e-49fd-8469-998f547d3a70.xml"}}, {"value": "2.91E-08", "module": "A1-A3"}, {"value": "2.4E-11", "module": "A4"}, {"value": "3.17E-08", "module": "A5"}, {"value": "0", "module": "B1"}, {"value": "0", "module": "B2"}, {"value": "0", "module": "B3"}, {"value": "0", "module": "B4"}, {"value": "0", "module": "B5"}, {"value": "0", "module": "B6"}, {"value": "0", "module": "B7"}, {"value": "0", "module": "C1"}, {"value": "3.98E-12", "module": "C2"}, {"value": "9.39E-12", "module": "C3"}, {"value": "1.7E-12", "module": "C4"}, {"value": "-1.53E-09", "module": "D"}]}}, {"referenceToLCIAMethodDataSet": {"shortDescription": [{"value": "Comparative toxic unit for humans (noncarcinogenic) (HTP-nc)", "lang": "en"}, {"value": "Toxizitätsvergleichseinheit für Menschen (nicht krebserregend) (HTP-nc)", "lang": "de"}], "type": "LCIA method data set", "refObjectId": "3af763a5-b7a1-48c9-9cee-1f223481fcef", "uri": "../lciamethods/3af763a5-b7a1-48c9-9cee-1f223481fcef.xml"}, "other": {"anies": [{"name": "referenceToUnitGroupDataSet", "value": {"shortDescription": [{"value": "CTUh", "lang": "en"}], "type": "unit group data set", "refObjectId": "d4c9523e-2d7e-49fd-8469-998f547d3a70", "uri": "../unitgroups/d4c9523e-2d7e-49fd-8469-998f547d3a70.xml"}}, {"value": "9.69E-08", "module": "A1-A3"}, {"value": "1.22E-09", "module": "A4"}, {"value": "8.62E-08", "module": "A5"}, {"value": "0", "module": "B1"}, {"value": "0", "module": "B2"}, {"value": "0", "module": "B3"}, {"value": "0", "module": "B4"}, {"value": "0", "module": "B5"}, {"value": "0", "module": "B6"}, {"value": "0", "module": "B7"}, {"value": "0", "module": "C1"}, {"value": "2.12E-10", "module": "C2"}, {"value": "6.77E-10", "module": "C3"}, {"value": "1.61E-10", "module": "C4"}, {"value": "-2.71E-08", "module": "D"}]}}, {"referenceToLCIAMethodDataSet": {"shortDescription": [{"value": "Soil quality index (SQP)", "lang": "en"}, {"value": "Bodenqualitätsindex (SQP)", "lang": "de"}], "type": "LCIA method data set", "refObjectId": "b2ad6890-c78d-11e6-9d9d-cec0c932ce01", "uri": "../lciamethods/b2ad6890-c78d-11e6-9d9d-cec0c932ce01.xml"}, "other": {"anies": [{"name": "referenceToUnitGroupDataSet", "value": {"shortDescription": [{"value": "SQP", "lang": "en"}], "type": "unit group data set", "refObjectId": "f130951c-e67f-4f7f-8dd4-665de3974e18", "uri": "../unitgroups/f130951c-e67f-4f7f-8dd4-665de3974e18.xml"}}, {"value": "20.5", "module": "A1-A3"}, {"value": "0.347", "module": "A4"}, {"value": "4.87", "module": "A5"}, {"value": "0", "module": "B1"}, {"value": "0", "module": "B2"}, {"value": "0", "module": "B3"}, {"value": "0", "module": "B4"}, {"value": "0", "module": "B5"}, {"value": "0", "module": "B6"}, {"value": "0", "module": "B7"}, {"value": "0", "module": "C1"}, {"value": "0.0911", "module": "C2"}, {"value": "0.162", "module": "C3"}, {"value": "0.00332", "module": "C4"}, {"value": "-7.22", "module": "D"}]}}]}, "otherAttributes": {"{http://www.indata.network/EPD/2019}epd-version": "1.2"}, "version": "1.1", "locations": "../ILCDLocations.xml"}