{"processInformation": {"dataSetInformation": {"UUID": "3d80fcc7-bc1a-42d1-b792-db2ff85f2417", "name": {"baseName": [{"value": "PerfectSense Lackplatten Span", "lang": "de"}, {"value": "PerfectSense Lacquered Chipboards", "lang": "en"}], "functionalUnitFlowProperties": [{"lang": "de"}]}, "classificationInformation": {"classification": [{"class": [{"value": "Holz", "level": 0, "classId": "3"}, {"value": "Holzwerkstoffe", "level": 1, "classId": "3.2"}, {"value": "Holzfaserplatten", "level": 2, "classId": "3.2.07"}], "name": "OEKOBAU.DAT"}, {"class": [{"value": "02 Bauprodukte", "level": 0}, {"value": "Holzwerkstoffe", "level": 1}, {"value": "Holzwerkstoffe", "level": 2}], "name": "IBUCategories"}]}, "generalComment": [{"value": "PerfectSense Lackplatten sind plattenfrmige Werkstoffe gem EN 312:2010-09, Spanplatten Anforderungen, welche fr allgemeine Zwecke im Trockenbereich klassifiziert sind.\n\nFr das Vorprodukt wird die Span-Trgerplatte gem EN 14322:2017-03, Holzwerkstoffe - Melaminbeschichtete Platten zur Verwendung im Innenbereich - Definition, Anforderungen und Klassifizierung mit einer Melaminharzbeschichtung versehen.\n\nEin spezielles Herstellungsverfahren ermglicht es, eine matte Oberflchenlackierung mit flachen oder tieferen Strukturen auf einem Spantrger zu kombinieren. Die Lackierung verleiht der PerfectSense Lackplatte Span eine samtig-matte Optik und Haptik mit Anti-Fingerprint Eigenschaft. Die PerfectSense Lackplatten werden standardmig mit einer einseitigen UV-Lackierung versehen*. Zum Schutz der lackierten Oberflche wird die PerfectSense Lackplatte mit einer Schutzfolie versehen, welche nach der endgltigen Verarbeitung von der Oberflche abgezogen wird.\n\n*Die optional verfgbare beidseitige Lackierung ist von der Gltigkeit dieser EPD ausgenommen.", "lang": "de"}, {"value": "PerfectSense Lacquered Boards are board-shaped materials according to EN 312:2010-09, Particleboard - Specification, which are classified for general purposes in dry conditions. \n\nFor the preliminary product, the chip coreboard is provided, according to the \nEN 14322:2017-03, Wood-based panels - Melamine faced boards for interior uses - Definition, requirements and classification with a melamine resin coat. \n\nA special manufacturing process makes it possible to combine a matt surface lacquer finish with flat or deeper texture on a chip coreboard. The lacquer finish gives PerfectSense Lacquered Chipboard a velvety matt look and feel with anti-fingerprint properties. PerfectSense Lacquered Boards are provided with a one-sided UV lacquer finish as standard*. \nTo protect the lacquered surface, the PerfectSense Lacquered Board is provided with a protective film, which is peeled off the surface after final processing. \n\n*The optionally available double-sided lacquer finish is excluded from the validity of this EPD.", "lang": "en"}]}, "quantitativeReference": {"referenceToReferenceFlow": [0]}, "time": {"referenceYear": 2023, "dataSetValidUntil": 2029, "other": {"anies": [{"name": "publicationDateOfEPD", "value": 1684281600000}]}}, "geography": {"locationOfOperationSupplyOrProduction": {"location": "DE"}}, "technology": {"technologyDescriptionAndIncludedProcesses": [{"value": "Als Basismaterial der PerfectSense Lackplatten Span dient eine melaminharzbeschichtete Spanplatte (EGGER Eurodekor Spanplatten beschichtet). Herstellung der Rohplatten (EGGER Eurospan): 1. Holzaufbereitung - Rundholzzerspanung - Hackschnitzelaufbereitung - Restholzaufbereitung 2. Trocknung der Späne auf ca. 2-3 % Restfeuchte 3. Sortierung der Späne 4. Beleimung der Späne 5. Streuung der beleimten Späne auf ein Formband 6. Verpressen des Spänekuchens in einer kontinuierlich arbeitenden Heißpresse (ContiRoll) 7. Formatierung der Rohplatten 8. Auskühlen der Rohplatten in Sternkühlwendern 9. Schleifen der Ober- und Unterseite 10. Abstapelung zu Großstapeln. Alle während der Produktion anfallenden Reste (Besäum-, Schneid- und Fräsreste) werden erneut dem Produktionsprozess zugeführt. Herstellung der Imprägnate für die Beschichtung: 1. Abwicklung der Rohpapiere 2. Aufnahme von Imprägnierharz (MUF) in der Anlage 3. Trocknung des imprägnierten Papiers in beheizten Trocknern 4. Formatierung des endlosen Papiers mittels Querschneider 5. Abstapelung der formatierten Bögen auf Paletten Beschichtung der Spanplatten (EGGER Eurodekor): 1. Legung der Imprägnate auf die Ober- und Unterseite der Rohplatte 2. Verpressung der Platte in der Heißpresse mit verschieden strukturierten Pressblechen 3. Qualitätssortierung und Abstapelung 4. Klimatisierungsphase von bis zu 14 Tagen Alle während der Beschichtung anfallenden Reste werden werksintern einer thermischen Verwertung zugeführt. Lackierung der beschichteten Spanplatte: 1. Lackierung mit Haftprimer, Aushärtung mittels UV-Strahlen 2. Lackierung mit Decklack als finale Oberfläche, Aushärtung mittels UV-Strahlen 3. Aufbringen der Schutzfolie 4. Qualitätssortierung und Abstapelung Am Produktionsstandort ist ein Qualitätsmanagementsystem nach den Anforderungen der ISO 9001 implementiert und zertifiziert. \nTechnische Daten: \nDie lackierte PerfectSense Platte hat eine melaminharzbeschichtete Spanplatte als Trgerplatte. Definition, Anforderung und Klassifizierung von melaminharzbeschichteten Platten zur Verwendung im Innenbereich sowie Matoleranzen liefert die Norm EN 14323. \n\nDie Oberflcheneigenschaften der lackierten Platte werden ber eine Vielzahl weiterer Normen geregelt, z.B. das Verhalten bei Kratzbeanspruchung nach EN 438-2 oder Oberflchenfehler laut AMK Merkblatt AMK-MB-009. \n\nDetaillierte Angaben entnehmen Sie bitte den Technischen Datenblttern, verfgbar auf www.egger.com. \nDeklarierte Einheit: \nDie vorliegende Umwelt-Produktdeklaration bezieht sich auf eine deklarierte Einheit von 1 m EGGER PerfectSense Lackplatten Span mit einem durchschnittlichen Flchengewicht von 12 kg/m.", "lang": "de"}, {"value": "The base material of PerfectSense Lacquered Chipboard is melamine-resin-coated chipboard (EGGER Eurodekor chipboard coated). Production of the raw boards (EGGER Eurospan): 1. Wood preparation - Roundwood cutting ­- Wood chip preparation ­- Waste wood treatment 2. Drying the chips to approximately 2 – 3 % residual moisture 3. Sorting the chips 4. Applying glue to the chips 5. Spreading the glue-coated chips onto a forming machine 6. Pressing the chip cake in a continuously operating hot press (ContiRoll) 7. Formatting of the raw boards 8. Cooling the raw boards in star coolers 9. Sanding the upper and lower sides 10. Stacking into large stacks. All scraps generated during production (trimming, cutting and milling scraps) are fed back into the production process. Production of impregnates for coating: 1. Processing the base paper 2. Addition of saturating resins (MUF) in the plant 3. Drying the impregnated paper in heated dryers 4. Formatting the endless paper by means of a cross-cutter 5. Stacking the formatted sheets on pallets Coating the chipboard (EGGER Eurodekor): 1. Laying the impregnated papers onto the upper and lower sides of the raw board 2. Pressing the board in the hot press with variously textured pressing sheets 3. Grading by quality and stacking 4. Acclimatisation phase of up to 14 days All waste generated in the course of the coating is used thermally within the plant. Lacquer finish of the coated chipboard: 1. Lacquering with adhesive primer, curing by means of UV rays 2. Lacquering with top coat as final surface, curing by means of UV rays 3. Application of protective film 4. Sorting by quality and stacking A quality management system in accordance with ISO 9001 requirements is implemented and certified at the production site. \nTechnical data: \nThe PerfectSense Lacquered Board has a melamine resin-coated chipboard as coreboard. The definition, requirement and classification of melamine faced boards for interior use and dimensional tolerances are provided by the EN 14323 standard. \n\nThe surface properties of the lacquered board are regulated by a number of other standards, e.g. the behaviour under scratching stress according to EN 438-2 or surface defects according to AMK leaflet AMK-MB-009. \n\nFor detailed information, please refer to the technical data sheets available at www.egger.com. \nDeclared unit: \nThis environmental product declaration refers to a declared unit of one square meter of EGGER PerfectSense Lacquered Chipboard produced with an average surface weight of 12 kg/m.", "lang": "en"}], "technologicalApplicability": [{"value": "PerfectSense Lackplatten Span werden vielseitig im Möbel- und Innenausbau eingesetzt wie zum Beispiel als Front, Schiebetür oder Korpusmaterial.", "lang": "de"}, {"value": "PerfectSense Lacquered Chipboard is used in a wide range of furniture and interior applications, for example, as a front, sliding door or body material.", "lang": "en"}]}}, "modellingAndValidation": {"LCIMethodAndAllocation": {"typeOfDataSet": "EPD", "referenceToLCAMethodDetails": [{"shortDescription": [{"value": "Holzwerkstoffe.pdf", "lang": "de"}], "type": "source data set", "refObjectId": "091dbd00-006b-4528-aebc-d6de5d7c96d2"}], "other": {"anies": [{"name": "subType", "value": "average dataset"}]}}, "dataSourcesTreatmentAndRepresentativeness": {"referenceToDataSource": [{"shortDescription": [{"value": "GaBi Database (all versions)", "lang": "de"}], "type": "source data set", "refObjectId": "28d74cc0-db8b-4d7e-bc44-5f6d56ce0c4a"}, {"shortDescription": [{"value": "GaBi Database Edition 2022, CUP 2022.02", "lang": "de"}], "type": "source data set", "refObjectId": "94f442cb-662e-43ea-a792-4b0a35132e93"}], "useAdviceForDataSet": [{"value": "Gültigkeitsbereich: \nDieses Dokument bezieht sich auf EGGER PerfectSense Span-Lackplatten, produziert in Brilon, Deutschland. \nSystemgrenze: \nDie kobilanz der EGGER PerfectSense Lackplatten Span beinhaltet eine cradle-to-gate (Wiege bis zum Werkstor) Betrachtung der auftretenden Umweltwirkungen mit den Modulen C1–C4 und Modul D (A1A3, +C, +D). Die folgenden Lebenszyklusphasen werden in der Analyse bercksichtigt:\n\nModul A1A3 | Produktionsstadium\nDas Produktionsstadium beinhaltet die Aufwendungen der Rohstoffversorgung (Rundholz, Herstellung der eingesetzten Basischemikalien fr die Leimsysteme der Holzwerkstoffe, die Komponenten der Imprgnierung wie Dekor- und Kraftpapier, Produktion der Lacke, Hilfsstoffe, etc.) sowie der damit verbundenen Transporte zum Produktionsstandort in Brilon. Innerhalb der Werksgrenzen werden der Holzplatz, die Nassspanaufbereitung, Trocknung, Beleimung, Streuung, Pressen, Schleifstrae bis zum Lager und Versand bercksichtigt. Die EURODEKOR Produkte werden darber hinaus durch das Aufbringen einer Imprgnierung in den Kurztaktpressen veredelt und anschlieend verpackt. Bei den PerfectSense Lackplatten Span werden die EURODEKOR Produkte zustzlich mit einer Lackschicht versehen. Das eingesetzte Leimsystem wird nicht am Standort hergestellt. Die Bereitstellung thermischer und elektrischer Energie, Druckluft und Wasser erfolgt durch zentrale Versorger am Standort Brilon. Der Groteil der eingesetzten elektrischen Energie wird vom deutschen Stromnetz bezogen. Im eigenen Biomasse-Kraftwerk wird sowohl internes Restholz als auch extern bezogenes Altholz verwertet. Die Systemgrenze fr in der Produktion verwendetes Altholz wird nach dem Sortieren und Hacken gesetzt. Dabei wird angenommen, dass das Ende der Abfalleigenschaft erreicht ist. Hier gilt die nach EN 15804 definierte Systemgrenze fr Sekundrrohstoffe.\n\nModul C1 | Rckbau/Abriss\nFr die PerfectSense Span-Lackplatte wurde ein manueller Ausbau angenommen. Die damit verbundenen Aufwnde sind vernachlssigbar, wodurch keine Umweltwirkungen aus dem Rckbau der Produkte deklariert werden.\n\nModul C2 | Transport zur Abfallbehandlung\nModul C2 beinhaltet den Transport zur Abfallbehandlung. Dazu wird der Transport via LKW ber 50 km Transportdistanz als reprsentatives Szenario angesetzt.\n\nModul C3 | Abfallbehandlung\nIn Modul C3 wird das Hacken nach Ausbau der Produkte betrachtet. Die Holzprodukte und mit ihnen die materialinhrenten Eigenschaften verlassen das Produktsystem als Sekundrbrennstoff in Modul C3.\n\nModul C4 | Beseitigung\nDas angesetzte Szenario deklariert die energetische Verwertung der Holzprodukte, wodurch keine Umweltauswirkungen aus der Abfallbehandlung der Produkte in C4 zu erwarten sind.\n\nModul D | Nutzen und Lasten auerhalb der Systemgrenze \nIn Modul D wird die energetische Verwertung des Produktes am Lebensende inklusive den entsprechenden energetischen Substitutionspotenzialen in Form eines europischen Durchschnittsszenarios beschrieben.", "lang": "de"}, {"value": "Scope: \nThis document refers to EGGER PerfectSense Lacquered Chipboard, produced in Brilon, Germany. \nSystem boundary: \nThe LCA of the EGGER PerfectSense Lacquered Chipboard includes a cradle-to-gate consideration of the occurring environmental impact with the modules C1-C4 and module D (A1-A3, +C, +D). The following life cycle phases are taken into account in the analysis: \n\nModule A1– A3 | Production stage \nThe production stage includes the expenses for the supply of raw materials (roundwood, production of the basic chemicals used for the gluing systems of the wood-based materials, the impregnation components such as decorative and kraft paper, production of the paint, auxiliary materials, etc.) and the associated transport to the production site in Brilon. Within the plant boundaries, the log yard, wet chip preparation, drying, gluing, spreading, pressing, the sanding line up to the warehouse and shipping are taken into account. The EURODEKOR products are also finished by applying an impregnation in the short-cycle presses and then packaged. In the case of PerfectSense Lacquered Chipboard, the EURODEKOR products are additionally coated with a paint layer. The glue system used is not manufactured on site. Thermal and electrical energy, compressed air and water are provided by central suppliers at the Brilon site. The majority of the electrical energy used is obtained from the German power grid. Both internal wood waste and scrap wood sourced externally are used in the in-house biomass power plant. The system boundary for the scrap wood used in the production is set after sorting and chopping. It is assumed that the end of the waste status has been reached. The system boundary for secondary raw materials according to EN 15804 applies. \n\nModule C1 | Dismantling / Demolition \nManual dismantling was assumed for the PerfectSense Lacquered Board. The associated efforts are negligible, which means that no environmental impact from the dismantling of the products is declared. \n\nModule C2 | Transport to waste treatment \nModule C2 includes transport to waste treatment. For this purpose, transport by lorry over a distance of 50 km is used as a representative scenario. \n\nModule C3 | Waste processing \nChopping after product disassembly is considered in module C3. The wood products and with them the material-inherent properties leave the product system as secondary fuel in module C3. \n\nModule C4 | Disposal \nThe scenario used declares the energy recovery of the wood products, which means that no environmental impact from the waste treatment of the products in C4 are to be expected. \n\nModule D | Uses and charges beyond the limits of the product system\nThe energy utilisation of the product at the end of its life cycle is described in Module D, including energetic substitution potentials as a European average scenario.", "lang": "en"}], "other": {"anies": [{"name": "referenceToOriginalEPD", "value": {"shortDescription": {"value": "PerfectSense Lackplatten Span.pdf", "defaultValue": "PerfectSense Lackplatten Span.pdf", "lstrings": [{"lang": "de", "value": "PerfectSense Lackplatten Span.pdf"}]}, "type": "source data set", "uuid": {"uuid": "c4d88650-3e83-4c72-852d-a751ba0b20a8"}, "refObjectId": "c4d88650-3e83-4c72-852d-a751ba0b20a8", "resourceURLs": ["https://oekobaudat.de/OEKOBAU.DAT/resource/sources/c4d88650-3e83-4c72-852d-a751ba0b20a8/PerfectSense_Lackplatten_Span_23562.pdf?version=00.03.000"]}}]}}, "validation": {"review": [{"referenceToNameOfReviewerAndInstitution": [{"shortDescription": [{"value": "Institut Bauen und Umwelt e. V.", "lang": "de"}], "type": "contact data set", "refObjectId": "d111dbec-b024-4be5-86c5-752d6eb2cf95", "uri": "../contacts/d111dbec-b024-4be5-86c5-752d6eb2cf95.xml"}], "type": "Accredited third party review"}]}, "complianceDeclarations": {"compliance": [{"referenceToComplianceSystem": {"shortDescription": [{"value": "DIN EN 15804+A2", "lang": "de"}], "type": "source data set", "refObjectId": "c0016b33-8cf7-415c-ac6e-deba0d21440d", "uri": "../sources/c0016b33-8cf7-415c-ac6e-deba0d21440d.xml"}}, {"referenceToComplianceSystem": {"shortDescription": [{"value": "ISO 14025", "lang": "de"}], "type": "source data set", "refObjectId": "4f2eb655-6e44-4874-a95a-e28f5442cd4d", "uri": "../sources/4f2eb655-6e44-4874-a95a-e28f5442cd4d.xml"}}]}}, "administrativeInformation": {"commissionerAndGoal": {"referenceToCommissioner": [{"shortDescription": [{"value": "Fritz EGGER GmbH & Co. OG", "lang": "de"}], "type": "contact data set", "refObjectId": "3ccb1a8b-2f9d-4de9-b22b-777128355981", "uri": "../contacts/3ccb1a8b-2f9d-4de9-b22b-777128355981.xml"}]}, "dataGenerator": {"referenceToPersonOrEntityGeneratingTheDataSet": [{"shortDescription": [{"value": "Daxner & Merl GmbH", "lang": "de"}], "type": "contact data set", "refObjectId": "ad8ad627-3991-42b7-a7ca-5a3fe0a34c28", "uri": "../contacts/ad8ad627-3991-42b7-a7ca-5a3fe0a34c28.xml"}]}, "dataEntryBy": {"timeStamp": 1684281600000, "referenceToDataSetFormat": [{"shortDescription": [{"value": "ILCD Format", "lang": "de"}], "type": "source data set", "refObjectId": "a97a0155-0234-4b87-b4ce-a45da52f2a40", "uri": "../sources/a97a0155-0234-4b87-b4ce-a45da52f2a40.xml"}, {"shortDescription": [{"value": "EPD-Datenformaterweiterungen v1.2", "lang": "de"}, {"value": "EPD Data Format Extensions v1.2", "lang": "en"}], "type": "source data set", "refObjectId": "a29449fd-aa2f-4de8-b5d7-4b06b43c6fde", "uri": "../sources/a29449fd-aa2f-4de8-b5d7-4b06b43c6fde.xml"}]}, "publicationAndOwnership": {"dataSetVersion": "00.09.000", "referenceToRegistrationAuthority": {"shortDescription": [{"value": "Institut Bauen und Umwelt e. V.", "lang": "de"}], "type": "contact data set", "refObjectId": "d111dbec-b024-4be5-86c5-752d6eb2cf95", "uri": "../contacts/d111dbec-b024-4be5-86c5-752d6eb2cf95.xml"}, "registrationNumber": "EPD-EGG-20200253-IBC4-DE", "referenceToOwnershipOfDataSet": {"shortDescription": [{"value": "Fritz EGGER GmbH & Co. OG", "lang": "de"}], "type": "contact data set", "refObjectId": "3ccb1a8b-2f9d-4de9-b22b-777128355981", "uri": "../contacts/3ccb1a8b-2f9d-4de9-b22b-777128355981.xml"}, "copyright": true, "licenseType": "Free of charge for all users and uses", "accessRestrictions": [{"value": "None", "lang": "en"}], "other": {"anies": [{"name": "referenceToPublisher", "value": {"shortDescription": [{"value": "Institut Bauen und Umwelt e. V.", "lang": "de"}], "type": "contact data set", "refObjectId": "d111dbec-b024-4be5-86c5-752d6eb2cf95", "uri": "../contacts/d111dbec-b024-4be5-86c5-752d6eb2cf95.xml"}}]}}}, "exchanges": {"exchange": [{"dataSetInternalID": 0, "referenceToFlowDataSet": {"shortDescription": [{"value": "PerfectSense Lackplatte Span (PerfectSense Lackplatte Span)", "lang": "de"}], "type": "flow data set", "refObjectId": "6d532f4d-0c5f-5d11-8803-79e7d0d19d54", "uri": "../flows/6d532f4d-0c5f-5d11-8803-79e7d0d19d54.xml"}, "meanAmount": 1.0, "referencesToDataSource": {}, "referenceFlow": true, "resolvedFlowVersion": "00.05.000", "resultingflowAmount": 1.0, "flowProperties": [{"name": [{"lang": "de", "value": "Fläche"}, {"lang": "en", "value": "Area"}], "uuid": "93a60a56-a3c8-19da-a746-0800200c9a66", "referenceFlowProperty": true, "meanValue": 1.0, "referenceUnit": "qm", "unitGroupUUID": "c20a03d7-bd90-4569-bc94-66cfd364dfc8"}], "materialProperties": [{"name": "layer thickness", "value": "0.028", "unit": "m", "unitDescription": "meters"}, {"name": "grammage", "value": "12.0", "unit": "kg/m^2", "unitDescription": "kilograms per square meter"}, {"name": "gross density", "value": "655.0", "unit": "kg/m^3", "unitDescription": "kilograms per cubic metre"}], "typeOfFlow": "Product flow", "classification": {"classHierarchy": "Holz / Holzwerkstoffe / Holzfaserplatten", "name": "OEKOBAU.DAT"}}, {"dataSetInternalID": 1, "referenceToFlowDataSet": {"shortDescription": [{"value": "Erneuerbare Primärenergie als Energieträger (PERE)", "lang": "de"}, {"value": "Renewable primary energy as energy carrier (PERE)", "lang": "en"}], "type": "flow data set", "refObjectId": "20f32be5-0398-4288-9b6d-accddd195317", "uri": "../flows/20f32be5-0398-4288-9b6d-accddd195317.xml"}, "exchange direction": "INPUT", "other": {"anies": [{"name": "referenceToUnitGroupDataSet", "value": {"shortDescription": [{"value": "MJ", "lang": "de"}], "type": "unit group data set", "refObjectId": "93a60a57-a3c8-11da-a746-0800200c9a66", "uri": "../unitgroups/93a60a57-a3c8-11da-a746-0800200c9a66.xml"}}, {"value": "124.706476901594", "module": "A1-A3"}, {"value": "0", "module": "C1"}, {"value": "0.0345986937228676", "module": "C2"}, {"value": "186.805876948131", "module": "C3"}, {"value": "0", "module": "C4"}, {"value": "-53.080727153405", "module": "D"}]}, "resolvedFlowVersion": "38.00.000", "flowProperties": [], "typeOfFlow": "Other flow", "classification": {"classHierarchy": "Quantities", "name": "GaBiCategories"}}, {"dataSetInternalID": 2, "referenceToFlowDataSet": {"shortDescription": [{"value": "Erneuerbare Primärenergie zur stofflichen Nutzung (PERM)", "lang": "de"}, {"value": "Renewable primary energy resources as material utilization (PERM)", "lang": "en"}], "type": "flow data set", "refObjectId": "fb3ec0de-548d-4508-aea5-00b73bf6f702", "uri": "../flows/fb3ec0de-548d-4508-aea5-00b73bf6f702.xml"}, "exchange direction": "INPUT", "other": {"anies": [{"name": "referenceToUnitGroupDataSet", "value": {"shortDescription": [{"value": "MJ", "lang": "de"}], "type": "unit group data set", "refObjectId": "93a60a57-a3c8-11da-a746-0800200c9a66", "uri": "../unitgroups/93a60a57-a3c8-11da-a746-0800200c9a66.xml"}}, {"value": "210.922248658611", "module": "A1-A3"}, {"value": "0", "module": "C1"}, {"value": "0", "module": "C2"}, {"value": "-185.8645714488", "module": "C3"}, {"value": "0", "module": "C4"}, {"value": "0", "module": "D"}]}, "resolvedFlowVersion": "38.00.000", "flowProperties": [], "typeOfFlow": "Other flow", "classification": {"classHierarchy": "Quantities", "name": "GaBiCategories"}}, {"dataSetInternalID": 3, "referenceToFlowDataSet": {"shortDescription": [{"value": "Total erneuerbare Primärenergie (PERT)", "lang": "de"}, {"value": "Total use of renewable primary energy resources (PERT)", "lang": "en"}], "type": "flow data set", "refObjectId": "53f97275-fa8a-4cdd-9024-65936002acd0", "uri": "../flows/53f97275-fa8a-4cdd-9024-65936002acd0.xml"}, "exchange direction": "INPUT", "other": {"anies": [{"name": "referenceToUnitGroupDataSet", "value": {"shortDescription": [{"value": "MJ", "lang": "de"}], "type": "unit group data set", "refObjectId": "93a60a57-a3c8-11da-a746-0800200c9a66", "uri": "../unitgroups/93a60a57-a3c8-11da-a746-0800200c9a66.xml"}}, {"value": "335.628725560205", "module": "A1-A3"}, {"value": "0", "module": "C1"}, {"value": "0.0345986937228676", "module": "C2"}, {"value": "0.941305499330498", "module": "C3"}, {"value": "0", "module": "C4"}, {"value": "-53.080727153405", "module": "D"}]}, "resolvedFlowVersion": "38.00.000", "flowProperties": [], "typeOfFlow": "Other flow", "classification": {"classHierarchy": "Quantities / Environmental quantities / EPD EN 15804 / LCI indicators", "name": "GaBiCategories"}}, {"dataSetInternalID": 4, "referenceToFlowDataSet": {"shortDescription": [{"value": "Nicht-erneuerbare Primärenergie als Energieträger (PENRE)", "lang": "de"}, {"value": "Non renewable primary energy as energy carrier (PENRE)", "lang": "en"}], "type": "flow data set", "refObjectId": "ac857178-2b45-46ec-892a-a9a4332f0372", "uri": "../flows/ac857178-2b45-46ec-892a-a9a4332f0372.xml"}, "exchange direction": "INPUT", "other": {"anies": [{"name": "referenceToUnitGroupDataSet", "value": {"shortDescription": [{"value": "MJ", "lang": "de"}], "type": "unit group data set", "refObjectId": "93a60a57-a3c8-11da-a746-0800200c9a66", "uri": "../unitgroups/93a60a57-a3c8-11da-a746-0800200c9a66.xml"}}, {"value": "70.1183597061999", "module": "A1-A3"}, {"value": "0", "module": "C1"}, {"value": "0.501168558196742", "module": "C2"}, {"value": "30.5742771716323", "module": "C3"}, {"value": "0", "module": "C4"}, {"value": "-168.107282344124", "module": "D"}]}, "resolvedFlowVersion": "38.00.000", "flowProperties": [], "typeOfFlow": "Other flow", "classification": {"classHierarchy": "Quantities", "name": "GaBiCategories"}}, {"dataSetInternalID": 5, "referenceToFlowDataSet": {"shortDescription": [{"value": "Nicht-erneuerbare Primärenergie zur stofflichen Nutzung (PENRM)", "lang": "de"}, {"value": "Non renewable primary energy as material utilization (PENRM)", "lang": "en"}], "type": "flow data set", "refObjectId": "1421caa0-679d-4bf4-b282-0eb850ccae27", "uri": "../flows/1421caa0-679d-4bf4-b282-0eb850ccae27.xml"}, "exchange direction": "INPUT", "other": {"anies": [{"name": "referenceToUnitGroupDataSet", "value": {"shortDescription": [{"value": "MJ", "lang": "de"}], "type": "unit group data set", "refObjectId": "93a60a57-a3c8-11da-a746-0800200c9a66", "uri": "../unitgroups/93a60a57-a3c8-11da-a746-0800200c9a66.xml"}}, {"value": "31.1338742744051", "module": "A1-A3"}, {"value": "0", "module": "C1"}, {"value": "0", "module": "C2"}, {"value": "-28.8772402744051", "module": "C3"}, {"value": "0", "module": "C4"}, {"value": "0", "module": "D"}]}, "resolvedFlowVersion": "38.00.000", "flowProperties": [], "typeOfFlow": "Other flow", "classification": {"classHierarchy": "Quantities", "name": "GaBiCategories"}}, {"dataSetInternalID": 6, "referenceToFlowDataSet": {"shortDescription": [{"value": "Total nicht erneuerbare Primärenergie (PENRT)", "lang": "de"}, {"value": "Total use of non renewable primary energy resources (PENRT)", "lang": "en"}], "type": "flow data set", "refObjectId": "06159210-646b-4c8d-8583-da9b3b95a6c1", "uri": "../flows/06159210-646b-4c8d-8583-da9b3b95a6c1.xml"}, "exchange direction": "INPUT", "other": {"anies": [{"name": "referenceToUnitGroupDataSet", "value": {"shortDescription": [{"value": "MJ", "lang": "de"}], "type": "unit group data set", "refObjectId": "93a60a57-a3c8-11da-a746-0800200c9a66", "uri": "../unitgroups/93a60a57-a3c8-11da-a746-0800200c9a66.xml"}}, {"value": "101.252233980605", "module": "A1-A3"}, {"value": "0", "module": "C1"}, {"value": "0.501168558196742", "module": "C2"}, {"value": "1.6970368972272", "module": "C3"}, {"value": "0", "module": "C4"}, {"value": "-168.107282344124", "module": "D"}]}, "resolvedFlowVersion": "38.00.000", "flowProperties": [], "typeOfFlow": "Other flow", "classification": {"classHierarchy": "Quantities / Environmental quantities / EPD EN 15804 / LCI indicators", "name": "GaBiCategories"}}, {"dataSetInternalID": 7, "referenceToFlowDataSet": {"shortDescription": [{"value": "Einsatz von Sekundärstoffen (SM)", "lang": "de"}, {"value": "Use of secondary material (SM)", "lang": "en"}], "type": "flow data set", "refObjectId": "c6a1f35f-2d09-4f54-8dfb-97e502e1ce92", "uri": "../flows/c6a1f35f-2d09-4f54-8dfb-97e502e1ce92.xml"}, "exchange direction": "INPUT", "other": {"anies": [{"name": "referenceToUnitGroupDataSet", "value": {"shortDescription": [{"value": "kg", "lang": "de"}], "type": "unit group data set", "refObjectId": "ad38d542-3fe9-439d-9b95-2f5f7752acaf", "uri": "../unitgroups/ad38d542-3fe9-439d-9b95-2f5f7752acaf.xml"}}, {"value": "5.19025154417363", "module": "A1-A3"}, {"value": "0", "module": "C1"}, {"value": "0", "module": "C2"}, {"value": "0", "module": "C3"}, {"value": "0", "module": "C4"}, {"value": "0", "module": "D"}]}, "resolvedFlowVersion": "38.00.000", "flowProperties": [], "typeOfFlow": "Other flow", "classification": {"classHierarchy": "Quantities / Environmental quantities / EPD EN 15804 / LCI indicators", "name": "GaBiCategories"}}, {"dataSetInternalID": 8, "referenceToFlowDataSet": {"shortDescription": [{"value": "Erneuerbare Sekundärbrennstoffe (RSF)", "lang": "de"}, {"value": "Use of renewable secondary fuels (RSF)", "lang": "en"}], "type": "flow data set", "refObjectId": "64333088-a55f-4aa2-9a31-c10b07816787", "uri": "../flows/64333088-a55f-4aa2-9a31-c10b07816787.xml"}, "exchange direction": "INPUT", "other": {"anies": [{"name": "referenceToUnitGroupDataSet", "value": {"shortDescription": [{"value": "MJ", "lang": "de"}], "type": "unit group data set", "refObjectId": "93a60a57-a3c8-11da-a746-0800200c9a66", "uri": "../unitgroups/93a60a57-a3c8-11da-a746-0800200c9a66.xml"}}, {"value": "13.0130922744352", "module": "A1-A3"}, {"value": "0", "module": "C1"}, {"value": "0", "module": "C2"}, {"value": "0", "module": "C3"}, {"value": "0", "module": "C4"}, {"value": "175.907540835471", "module": "D"}]}, "resolvedFlowVersion": "38.00.000", "flowProperties": [], "typeOfFlow": "Other flow", "classification": {"classHierarchy": "Quantities / Environmental quantities / EPD EN 15804 / LCI indicators", "name": "GaBiCategories"}}, {"dataSetInternalID": 9, "referenceToFlowDataSet": {"shortDescription": [{"value": "Nicht erneuerbare Sekundärbrennstoffe (NRSF)", "lang": "de"}, {"value": "Use of non renewable secondary fuels (NRSF)", "lang": "en"}], "type": "flow data set", "refObjectId": "89def144-d39a-4287-b86f-efde453ddcb2", "uri": "../flows/89def144-d39a-4287-b86f-efde453ddcb2.xml"}, "exchange direction": "INPUT", "other": {"anies": [{"name": "referenceToUnitGroupDataSet", "value": {"shortDescription": [{"value": "MJ", "lang": "de"}], "type": "unit group data set", "refObjectId": "93a60a57-a3c8-11da-a746-0800200c9a66", "uri": "../unitgroups/93a60a57-a3c8-11da-a746-0800200c9a66.xml"}}, {"value": "0", "module": "A1-A3"}, {"value": "0", "module": "C1"}, {"value": "0", "module": "C2"}, {"value": "0", "module": "C3"}, {"value": "0", "module": "C4"}, {"value": "26.6636539119072", "module": "D"}]}, "resolvedFlowVersion": "38.00.000", "flowProperties": [], "typeOfFlow": "Other flow", "classification": {"classHierarchy": "Quantities / Environmental quantities / EPD EN 15804 / LCI indicators", "name": "GaBiCategories"}}, {"dataSetInternalID": 10, "referenceToFlowDataSet": {"shortDescription": [{"value": "Einsatz von Süßwasserressourcen (FW)", "lang": "de"}, {"value": "Use of net fresh water (FW)", "lang": "en"}], "type": "flow data set", "refObjectId": "3cf952c8-f3a4-461d-8c96-96456ca62246", "uri": "../flows/3cf952c8-f3a4-461d-8c96-96456ca62246.xml"}, "exchange direction": "INPUT", "other": {"anies": [{"name": "referenceToUnitGroupDataSet", "value": {"shortDescription": [{"value": "m^3", "lang": "de"}], "type": "unit group data set", "refObjectId": "cd950537-0a98-4044-9ba7-9f9a68d0a504", "uri": "../unitgroups/cd950537-0a98-4044-9ba7-9f9a68d0a504.xml"}}, {"value": "0.0176050544871105", "module": "A1-A3"}, {"value": "0", "module": "C1"}, {"value": "3.99676773761943E-05", "module": "C2"}, {"value": "0.00089795466080228", "module": "C3"}, {"value": "0", "module": "C4"}, {"value": "-0.0353098048402671", "module": "D"}]}, "resolvedFlowVersion": "38.00.000", "flowProperties": [], "typeOfFlow": "Other flow", "classification": {"classHierarchy": "Quantities / Environmental quantities / EPD EN 15804 / LCI indicators", "name": "GaBiCategories"}}, {"dataSetInternalID": 11, "referenceToFlowDataSet": {"shortDescription": [{"value": "Gefährlicher Abfall zur Deponie (HWD)", "lang": "de"}, {"value": "Hazardous waste disposed (HWD)", "lang": "en"}], "type": "flow data set", "refObjectId": "430f9e0f-59b2-46a0-8e0d-55e0e84948fc", "uri": "../flows/430f9e0f-59b2-46a0-8e0d-55e0e84948fc.xml"}, "exchange direction": "OUTPUT", "other": {"anies": [{"name": "referenceToUnitGroupDataSet", "value": {"shortDescription": [{"value": "kg", "lang": "de"}], "type": "unit group data set", "refObjectId": "ad38d542-3fe9-439d-9b95-2f5f7752acaf", "uri": "../unitgroups/ad38d542-3fe9-439d-9b95-2f5f7752acaf.xml"}}, {"value": "7.13097053349953E-06", "module": "A1-A3"}, {"value": "0", "module": "C1"}, {"value": "2.65178404281239E-12", "module": "C2"}, {"value": "1.46751336338787E-10", "module": "C3"}, {"value": "0", "module": "C4"}, {"value": "-1.03445611815334E-08", "module": "D"}]}, "resolvedFlowVersion": "38.00.000", "flowProperties": [], "typeOfFlow": "Other flow", "classification": {"classHierarchy": "Quantities / Environmental quantities / EPD EN 15804 / LCI indicators", "name": "GaBiCategories"}}, {"dataSetInternalID": 12, "referenceToFlowDataSet": {"shortDescription": [{"value": "Entsorgter nicht gefährlicher Abfall (NHWD)", "lang": "de"}, {"value": "Non hazardous waste disposed (NHWD)", "lang": "en"}], "type": "flow data set", "refObjectId": "b29ef66b-e286-4afa-949f-62f1a7b4d7fa", "uri": "../flows/b29ef66b-e286-4afa-949f-62f1a7b4d7fa.xml"}, "exchange direction": "OUTPUT", "other": {"anies": [{"name": "referenceToUnitGroupDataSet", "value": {"shortDescription": [{"value": "kg", "lang": "de"}], "type": "unit group data set", "refObjectId": "ad38d542-3fe9-439d-9b95-2f5f7752acaf", "uri": "../unitgroups/ad38d542-3fe9-439d-9b95-2f5f7752acaf.xml"}}, {"value": "0.108609024325726", "module": "A1-A3"}, {"value": "0", "module": "C1"}, {"value": "8.16528296828049E-05", "module": "C2"}, {"value": "0.00127761573806988", "module": "C3"}, {"value": "0", "module": "C4"}, {"value": "0.00408844471964961", "module": "D"}]}, "resolvedFlowVersion": "38.00.000", "flowProperties": [], "typeOfFlow": "Other flow", "classification": {"classHierarchy": "Quantities / Environmental quantities / EPD EN 15804 / LCI indicators", "name": "GaBiCategories"}}, {"dataSetInternalID": 13, "referenceToFlowDataSet": {"shortDescription": [{"value": "Entsorgter radioaktiver Abfall (RWD)", "lang": "de"}, {"value": "Radioactive waste disposed (RWD)", "lang": "en"}], "type": "flow data set", "refObjectId": "3449546e-52ad-4b39-b809-9fb77cea8ff6", "uri": "../flows/3449546e-52ad-4b39-b809-9fb77cea8ff6.xml"}, "exchange direction": "OUTPUT", "other": {"anies": [{"name": "referenceToUnitGroupDataSet", "value": {"shortDescription": [{"value": "kg", "lang": "de"}], "type": "unit group data set", "refObjectId": "ad38d542-3fe9-439d-9b95-2f5f7752acaf", "uri": "../unitgroups/ad38d542-3fe9-439d-9b95-2f5f7752acaf.xml"}}, {"value": "0.00238978710266757", "module": "A1-A3"}, {"value": "0", "module": "C1"}, {"value": "9.30313294297566E-07", "module": "C2"}, {"value": "0.000271050118461283", "module": "C3"}, {"value": "0", "module": "C4"}, {"value": "-0.0152418795259343", "module": "D"}]}, "resolvedFlowVersion": "38.00.000", "flowProperties": [], "typeOfFlow": "Other flow", "classification": {"classHierarchy": "Quantities / Environmental quantities / EPD EN 15804 / LCI indicators", "name": "GaBiCategories"}}, {"dataSetInternalID": 14, "referenceToFlowDataSet": {"shortDescription": [{"value": "Komponenten für die Wiederverwendung (CRU)", "lang": "de"}, {"value": "Components for re-use (CRU)", "lang": "en"}], "type": "flow data set", "refObjectId": "a2b32f97-3fc7-4af2-b209-525bc6426f33", "uri": "../flows/a2b32f97-3fc7-4af2-b209-525bc6426f33.xml"}, "exchange direction": "OUTPUT", "other": {"anies": [{"name": "referenceToUnitGroupDataSet", "value": {"shortDescription": [{"value": "kg", "lang": "de"}], "type": "unit group data set", "refObjectId": "ad38d542-3fe9-439d-9b95-2f5f7752acaf", "uri": "../unitgroups/ad38d542-3fe9-439d-9b95-2f5f7752acaf.xml"}}, {"value": "0", "module": "A1-A3"}, {"value": "0", "module": "C1"}, {"value": "0", "module": "C2"}, {"value": "0", "module": "C3"}, {"value": "0", "module": "C4"}, {"value": "0", "module": "D"}]}, "resolvedFlowVersion": "38.00.000", "flowProperties": [], "typeOfFlow": "Other flow", "classification": {"classHierarchy": "Quantities / Environmental quantities / EPD EN 15804 / LCI indicators", "name": "GaBiCategories"}}, {"dataSetInternalID": 15, "referenceToFlowDataSet": {"shortDescription": [{"value": "Stoffe zum Recycling (MFR)", "lang": "de"}, {"value": "Materials for recycling (MFR)", "lang": "en"}], "type": "flow data set", "refObjectId": "d7fe48a5-4103-49c8-9aae-b0b5dfdbd6ae", "uri": "../flows/d7fe48a5-4103-49c8-9aae-b0b5dfdbd6ae.xml"}, "exchange direction": "OUTPUT", "other": {"anies": [{"name": "referenceToUnitGroupDataSet", "value": {"shortDescription": [{"value": "kg", "lang": "de"}], "type": "unit group data set", "refObjectId": "ad38d542-3fe9-439d-9b95-2f5f7752acaf", "uri": "../unitgroups/ad38d542-3fe9-439d-9b95-2f5f7752acaf.xml"}}, {"value": "0", "module": "A1-A3"}, {"value": "0", "module": "C1"}, {"value": "0", "module": "C2"}, {"value": "0", "module": "C3"}, {"value": "0", "module": "C4"}, {"value": "0", "module": "D"}]}, "resolvedFlowVersion": "38.00.000", "flowProperties": [], "typeOfFlow": "Other flow", "classification": {"classHierarchy": "Quantities / Environmental quantities / EPD EN 15804 / LCI indicators", "name": "GaBiCategories"}}, {"dataSetInternalID": 16, "referenceToFlowDataSet": {"shortDescription": [{"value": "Stoffe für die Energierückgewinnung (MER)", "lang": "de"}, {"value": "Materials for energy recovery (MER)", "lang": "en"}], "type": "flow data set", "refObjectId": "59a9181c-3aaf-46ee-8b13-2b3723b6e447", "uri": "../flows/59a9181c-3aaf-46ee-8b13-2b3723b6e447.xml"}, "exchange direction": "OUTPUT", "other": {"anies": [{"name": "referenceToUnitGroupDataSet", "value": {"shortDescription": [{"value": "kg", "lang": "de"}], "type": "unit group data set", "refObjectId": "ad38d542-3fe9-439d-9b95-2f5f7752acaf", "uri": "../unitgroups/ad38d542-3fe9-439d-9b95-2f5f7752acaf.xml"}}, {"value": "0", "module": "A1-A3"}, {"value": "0", "module": "C1"}, {"value": "0", "module": "C2"}, {"value": "12.6644528301887", "module": "C3"}, {"value": "0", "module": "C4"}, {"value": "0", "module": "D"}]}, "resolvedFlowVersion": "38.00.000", "flowProperties": [], "typeOfFlow": "Other flow", "classification": {"classHierarchy": "Quantities / Environmental quantities / EPD EN 15804 / LCI indicators", "name": "GaBiCategories"}}, {"dataSetInternalID": 17, "referenceToFlowDataSet": {"shortDescription": [{"value": "Exportierte elektrische Energie (EEE)", "lang": "de"}, {"value": "Exported electrical energy (EEE)", "lang": "en"}], "type": "flow data set", "refObjectId": "4da0c987-2b76-40d6-9e9e-82a017aaaf29", "uri": "../flows/4da0c987-2b76-40d6-9e9e-82a017aaaf29.xml"}, "exchange direction": "OUTPUT", "other": {"anies": [{"name": "referenceToUnitGroupDataSet", "value": {"shortDescription": [{"value": "MJ", "lang": "de"}], "type": "unit group data set", "refObjectId": "93a60a57-a3c8-11da-a746-0800200c9a66", "uri": "../unitgroups/93a60a57-a3c8-11da-a746-0800200c9a66.xml"}}, {"value": "0", "module": "A1-A3"}, {"value": "0", "module": "C1"}, {"value": "0", "module": "C2"}, {"value": "0", "module": "C3"}, {"value": "0", "module": "C4"}, {"value": "0", "module": "D"}]}, "resolvedFlowVersion": "38.00.000", "flowProperties": [], "typeOfFlow": "Other flow", "classification": {"classHierarchy": "Quantities / Environmental quantities / EPD EN 15804 / LCI indicators", "name": "GaBiCategories"}}, {"dataSetInternalID": 18, "referenceToFlowDataSet": {"shortDescription": [{"value": "Exportierte thermische Energie (EET)", "lang": "de"}, {"value": "Exported thermal energy (EET)", "lang": "en"}], "type": "flow data set", "refObjectId": "98daf38a-7a79-46d3-9a37-2b7bd0955810", "uri": "../flows/98daf38a-7a79-46d3-9a37-2b7bd0955810.xml"}, "exchange direction": "OUTPUT", "other": {"anies": [{"name": "referenceToUnitGroupDataSet", "value": {"shortDescription": [{"value": "MJ", "lang": "de"}], "type": "unit group data set", "refObjectId": "93a60a57-a3c8-11da-a746-0800200c9a66", "uri": "../unitgroups/93a60a57-a3c8-11da-a746-0800200c9a66.xml"}}, {"value": "0", "module": "A1-A3"}, {"value": "0", "module": "C1"}, {"value": "0", "module": "C2"}, {"value": "0", "module": "C3"}, {"value": "0", "module": "C4"}, {"value": "0", "module": "D"}]}, "resolvedFlowVersion": "38.00.000", "flowProperties": [], "typeOfFlow": "Other flow", "classification": {"classHierarchy": "Quantities / Environmental quantities / EPD EN 15804 / LCI indicators", "name": "GaBiCategories"}}]}, "LCIAResults": {"LCIAResult": [{"referenceToLCIAMethodDataSet": {"shortDescription": [{"value": "Globales Erwärmungspotenzial total (GWP-total)", "lang": "de"}, {"value": "Global Warming Potential total (GWP-total)", "lang": "en"}], "type": "LCIA method data set", "refObjectId": "6a37f984-a4b3-458a-a20a-64418c145fa2", "uri": "../lciamethods/6a37f984-a4b3-458a-a20a-64418c145fa2.xml"}, "other": {"anies": [{"name": "referenceToUnitGroupDataSet", "value": {"shortDescription": [{"value": "kg CO_(2)-Äq.", "lang": "de"}], "type": "unit group data set", "refObjectId": "1ebf3012-d0db-4de2-aefd-ef30cedb0be1", "uri": "../unitgroups/1ebf3012-d0db-4de2-aefd-ef30cedb0be1.xml"}}, {"value": "-13.5388948912472", "module": "A1-A3"}, {"value": "0", "module": "C1"}, {"value": "0.038010644791635", "module": "C2"}, {"value": "18.5291570429222", "module": "C3"}, {"value": "0", "module": "C4"}, {"value": "-8.48658396520291", "module": "D"}]}}, {"referenceToLCIAMethodDataSet": {"shortDescription": [{"value": "Globales Erwärmungspotenzial fossil (GWP-fossil)", "lang": "de"}, {"value": "Global Warming Potential fossil fuels (GWP-fossil)", "lang": "en"}], "type": "LCIA method data set", "refObjectId": "5f635281-343e-44fb-83df-1971b155e6b6", "uri": "../lciamethods/5f635281-343e-44fb-83df-1971b155e6b6.xml"}, "other": {"anies": [{"name": "referenceToUnitGroupDataSet", "value": {"shortDescription": [{"value": "kg CO_(2)-Äq.", "lang": "de"}], "type": "unit group data set", "refObjectId": "1ebf3012-d0db-4de2-aefd-ef30cedb0be1", "uri": "../unitgroups/1ebf3012-d0db-4de2-aefd-ef30cedb0be1.xml"}}, {"value": "4.77250103528591", "module": "A1-A3"}, {"value": "0", "module": "C1"}, {"value": "0.0381262071676065", "module": "C2"}, {"value": "0.0934670412285459", "module": "C3"}, {"value": "0", "module": "C4"}, {"value": "-8.43002177442585", "module": "D"}]}}, {"referenceToLCIAMethodDataSet": {"shortDescription": [{"value": "Globales Erwärmungspotenzial biogen (GWP-biogenic)", "lang": "de"}, {"value": "Global Warming Potential biogenic (GWP-biogenic)", "lang": "en"}], "type": "LCIA method data set", "refObjectId": "2356e1ab-0185-4db5-86e5-16de51c7485c", "uri": "../lciamethods/2356e1ab-0185-4db5-86e5-16de51c7485c.xml"}, "other": {"anies": [{"name": "referenceToUnitGroupDataSet", "value": {"shortDescription": [{"value": "kg CO_(2)-Äq.", "lang": "de"}], "type": "unit group data set", "refObjectId": "1ebf3012-d0db-4de2-aefd-ef30cedb0be1", "uri": "../unitgroups/1ebf3012-d0db-4de2-aefd-ef30cedb0be1.xml"}}, {"value": "-18.3146262002107", "module": "A1-A3"}, {"value": "0", "module": "C1"}, {"value": "-0.000371810591402307", "module": "C2"}, {"value": "18.4356702386558", "module": "C3"}, {"value": "0", "module": "C4"}, {"value": "-0.0553766161608529", "module": "D"}]}}, {"referenceToLCIAMethodDataSet": {"shortDescription": [{"value": "Globales Erwärmungspotenzial luluc (GWP-luluc)", "lang": "de"}, {"value": "Global Warming Potential luluc (GWP-luluc)", "lang": "en"}], "type": "LCIA method data set", "refObjectId": "4331bbdb-978a-490d-8707-eeb047f01a55", "uri": "../lciamethods/4331bbdb-978a-490d-8707-eeb047f01a55.xml"}, "other": {"anies": [{"name": "referenceToUnitGroupDataSet", "value": {"shortDescription": [{"value": "kg CO_(2)-Äq.", "lang": "de"}], "type": "unit group data set", "refObjectId": "1ebf3012-d0db-4de2-aefd-ef30cedb0be1", "uri": "../unitgroups/1ebf3012-d0db-4de2-aefd-ef30cedb0be1.xml"}}, {"value": "0.00323027367763115", "module": "A1-A3"}, {"value": "0", "module": "C1"}, {"value": "0.000256248215430725", "module": "C2"}, {"value": "1.97630379164736E-05", "module": "C3"}, {"value": "0", "module": "C4"}, {"value": "-0.0011855746162048", "module": "D"}]}}, {"referenceToLCIAMethodDataSet": {"shortDescription": [{"value": "Abbau Potential der stratosphärischen Ozonschicht (ODP)", "lang": "de"}, {"value": "Depletion potential of the stratospheric ozone layer (ODP)", "lang": "en"}], "type": "LCIA method data set", "refObjectId": "b5c629d6-def3-11e6-bf01-fe55135034f3", "uri": "../lciamethods/b5c629d6-def3-11e6-bf01-fe55135034f3.xml"}, "other": {"anies": [{"name": "referenceToUnitGroupDataSet", "value": {"shortDescription": [{"value": "kg CFC11-Äq.", "lang": "de"}], "type": "unit group data set", "refObjectId": "d9e957c9-7309-4474-bf3a-7777df6c4e5b", "uri": "../unitgroups/d9e957c9-7309-4474-bf3a-7777df6c4e5b.xml"}}, {"value": "6.29934583761955E-11", "module": "A1-A3"}, {"value": "0", "module": "C1"}, {"value": "3.73429871205722E-15", "module": "C2"}, {"value": "1.36786816940539E-12", "module": "C3"}, {"value": "0", "module": "C4"}, {"value": "-7.69893396668678E-11", "module": "D"}]}}, {"referenceToLCIAMethodDataSet": {"shortDescription": [{"value": "Versauerungspotenzial von Boden und Wasser (AP)", "lang": "de"}, {"value": "Acidification potential of land and water (AP)", "lang": "en"}], "type": "LCIA method data set", "refObjectId": "b5c611c6-def3-11e6-bf01-fe55135034f3", "uri": "../lciamethods/b5c611c6-def3-11e6-bf01-fe55135034f3.xml"}, "other": {"anies": [{"name": "referenceToUnitGroupDataSet", "value": {"shortDescription": [{"value": "mol H^(+)-Äq.", "lang": "de"}], "type": "unit group data set", "refObjectId": "42e089ac-92bf-4bf2-8ca1-5fc40d18f2ed", "uri": "../unitgroups/42e089ac-92bf-4bf2-8ca1-5fc40d18f2ed.xml"}}, {"value": "0.0112549131600262", "module": "A1-A3"}, {"value": "0", "module": "C1"}, {"value": "0.000127081776680894", "module": "C2"}, {"value": "0.000205188229236694", "module": "C3"}, {"value": "0", "module": "C4"}, {"value": "0.00865437581684908", "module": "D"}]}}, {"referenceToLCIAMethodDataSet": {"shortDescription": [{"value": "Eutrophierungspotenzial Süßwasser (EP-freshwater)", "lang": "de"}, {"value": "Eutrophication potential aquatic freshwater (EP-freshwater)", "lang": "en"}], "type": "LCIA method data set", "refObjectId": "b53ec18f-7377-4ad3-86eb-cc3f4f276b2b", "uri": "../lciamethods/b53ec18f-7377-4ad3-86eb-cc3f4f276b2b.xml"}, "other": {"anies": [{"name": "referenceToUnitGroupDataSet", "value": {"shortDescription": [{"value": "kg P-Äq.", "lang": "de"}], "type": "unit group data set", "refObjectId": "0429039d-a61d-4590-ba67-aa4a20a810a1", "uri": "../unitgroups/0429039d-a61d-4590-ba67-aa4a20a810a1.xml"}}, {"value": "1.57567550914654E-05", "module": "A1-A3"}, {"value": "0", "module": "C1"}, {"value": "1.3584396077302E-07", "module": "C2"}, {"value": "2.72689954945762E-07", "module": "C3"}, {"value": "0", "module": "C4"}, {"value": "-1.5488881982776E-05", "module": "D"}]}}, {"referenceToLCIAMethodDataSet": {"shortDescription": [{"value": "Eutrophierungspotenzial Salzwasser (EP-marine)", "lang": "de"}, {"value": "Eutrophication potential aquatic marine (EP-marine)", "lang": "en"}], "type": "LCIA method data set", "refObjectId": "b5c619fa-def3-11e6-bf01-fe55135034f3", "uri": "../lciamethods/b5c619fa-def3-11e6-bf01-fe55135034f3.xml"}, "other": {"anies": [{"name": "referenceToUnitGroupDataSet", "value": {"shortDescription": [{"value": "kg N-Äq.", "lang": "de"}], "type": "unit group data set", "refObjectId": "d05bb823-ecdf-4686-8c40-bf1d9257859f", "uri": "../unitgroups/d05bb823-ecdf-4686-8c40-bf1d9257859f.xml"}}, {"value": "0.00462553824133892", "module": "A1-A3"}, {"value": "0", "module": "C1"}, {"value": "5.81077645261426E-05", "module": "C2"}, {"value": "4.60365490317834E-05", "module": "C3"}, {"value": "0", "module": "C4"}, {"value": "0.00204361928418146", "module": "D"}]}}, {"referenceToLCIAMethodDataSet": {"shortDescription": [{"value": "Eutrophierungspotenzial Land (EP-terrestrial)", "lang": "de"}, {"value": "Eutrophication potential terrestrial (EP-terrestrial)", "lang": "en"}], "type": "LCIA method data set", "refObjectId": "b5c614d2-def3-11e6-bf01-fe55135034f3", "uri": "../lciamethods/b5c614d2-def3-11e6-bf01-fe55135034f3.xml"}, "other": {"anies": [{"name": "referenceToUnitGroupDataSet", "value": {"shortDescription": [{"value": "mol N-Äq.", "lang": "de"}], "type": "unit group data set", "refObjectId": "71b4d617-0ec9-4d3f-b65e-e438940c2401", "uri": "../unitgroups/71b4d617-0ec9-4d3f-b65e-e438940c2401.xml"}}, {"value": "0.0413927226934754", "module": "A1-A3"}, {"value": "0", "module": "C1"}, {"value": "0.000650799948331944", "module": "C2"}, {"value": "0.000482983842160717", "module": "C3"}, {"value": "0", "module": "C4"}, {"value": "0.0239618665576726", "module": "D"}]}}, {"referenceToLCIAMethodDataSet": {"shortDescription": [{"value": "Bildungspotential für troposphärisches Ozon (POCP)", "lang": "de"}, {"value": "Formation potential of tropospheric ozone photochemical oxidants (POCP)", "lang": "en"}], "type": "LCIA method data set", "refObjectId": "b5c610fe-def3-11e6-bf01-fe55135034f3", "uri": "../lciamethods/b5c610fe-def3-11e6-bf01-fe55135034f3.xml"}, "other": {"anies": [{"name": "referenceToUnitGroupDataSet", "value": {"shortDescription": [{"value": "kg NMVOC-Äq.", "lang": "de"}], "type": "unit group data set", "refObjectId": "d27c25f8-fbc1-44c6-b47b-4adbae4199c6", "uri": "../unitgroups/d27c25f8-fbc1-44c6-b47b-4adbae4199c6.xml"}}, {"value": "0.0092697252958337", "module": "A1-A3"}, {"value": "0", "module": "C1"}, {"value": "0.000114071041555922", "module": "C2"}, {"value": "0.00012446633259556", "module": "C3"}, {"value": "0", "module": "C4"}, {"value": "0.00848386316263545", "module": "D"}]}}, {"referenceToLCIAMethodDataSet": {"shortDescription": [{"value": "Potenzial für den abiotischen Abbau nicht fossiler Ressourcen (ADPE)", "lang": "de"}, {"value": "Abiotic depletion potential for non fossil resources (ADPE)", "lang": "en"}], "type": "LCIA method data set", "refObjectId": "b2ad6494-c78d-11e6-9d9d-cec0c932ce01", "uri": "../lciamethods/b2ad6494-c78d-11e6-9d9d-cec0c932ce01.xml"}, "other": {"anies": [{"name": "referenceToUnitGroupDataSet", "value": {"shortDescription": [{"value": "kg Sb-Äq.", "lang": "de"}], "type": "unit group data set", "refObjectId": "54ccd2d9-a32a-4fc2-923d-f2c8c93e89d4", "uri": "../unitgroups/54ccd2d9-a32a-4fc2-923d-f2c8c93e89d4.xml"}}, {"value": "2.15831604816377E-06", "module": "A1-A3"}, {"value": "0", "module": "C1"}, {"value": "3.83278193204386E-09", "module": "C2"}, {"value": "2.54651030172623E-08", "module": "C3"}, {"value": "0", "module": "C4"}, {"value": "-1.63848543666997E-06", "module": "D"}]}}, {"referenceToLCIAMethodDataSet": {"shortDescription": [{"value": "Potenzial für den abiotischen Abbau fossiler Brennstoffe (ADPF)", "lang": "de"}, {"value": "Abiotic depletion potential for fossil resources (ADPF)", "lang": "en"}], "type": "LCIA method data set", "refObjectId": "b2ad6110-c78d-11e6-9d9d-cec0c932ce01", "uri": "../lciamethods/b2ad6110-c78d-11e6-9d9d-cec0c932ce01.xml"}, "other": {"anies": [{"name": "referenceToUnitGroupDataSet", "value": {"shortDescription": [{"value": "MJ", "lang": "de"}], "type": "unit group data set", "refObjectId": "93a60a57-a3c8-11da-a746-0800200c9a66", "uri": "../unitgroups/93a60a57-a3c8-11da-a746-0800200c9a66.xml"}}, {"value": "101.215382192", "module": "A1-A3"}, {"value": "0", "module": "C1"}, {"value": "0.49919187490445", "module": "C2"}, {"value": "1.6966005487772", "module": "C3"}, {"value": "0", "module": "C4"}, {"value": "-168.081836071476", "module": "D"}]}}, {"referenceToLCIAMethodDataSet": {"shortDescription": [{"value": "Wassernutzung (WDP)", "lang": "de"}, {"value": "Water use (WDP)", "lang": "en"}], "type": "LCIA method data set", "refObjectId": "b2ad66ce-c78d-11e6-9d9d-cec0c932ce01", "uri": "../lciamethods/b2ad66ce-c78d-11e6-9d9d-cec0c932ce01.xml"}, "other": {"anies": [{"name": "referenceToUnitGroupDataSet", "value": {"shortDescription": [{"value": "m^(3) Welt-Äq. entzogen", "lang": "de"}], "type": "unit group data set", "refObjectId": "6ae2df01-888e-46c8-b17d-49fa3869b476", "uri": "../unitgroups/6ae2df01-888e-46c8-b17d-49fa3869b476.xml"}}, {"value": "0.236781370777695", "module": "A1-A3"}, {"value": "0", "module": "C1"}, {"value": "0.000425460763433604", "module": "C2"}, {"value": "0.0213121696559737", "module": "C3"}, {"value": "0", "module": "C4"}, {"value": "-0.537922747189668", "module": "D"}]}}, {"referenceToLCIAMethodDataSet": {"shortDescription": [{"value": "Auftreten von Krankheiten aufgrund von Feinstaubemissionen (PM)", "lang": "de"}, {"value": "Incidence of disease due to PM emissions (PM)", "lang": "en"}], "type": "LCIA method data set", "refObjectId": "b5c602c6-def3-11e6-bf01-fe55135034f3", "uri": "../lciamethods/b5c602c6-def3-11e6-bf01-fe55135034f3.xml"}, "other": {"anies": [{"name": "referenceToUnitGroupDataSet", "value": {"shortDescription": [{"value": "Krankheitsfälle", "lang": "de"}], "type": "unit group data set", "refObjectId": "3883559b-648f-4afc-8ba2-0bd24f3affa3", "uri": "../unitgroups/3883559b-648f-4afc-8ba2-0bd24f3affa3.xml"}}, {"value": "1.13305833628856E-07", "module": "A1-A3"}, {"value": "0", "module": "C1"}, {"value": "7.27225313039126E-10", "module": "C2"}, {"value": "1.70088564310215E-09", "module": "C3"}, {"value": "0", "module": "C4"}, {"value": "-2.01416742894978E-08", "module": "D"}]}}, {"referenceToLCIAMethodDataSet": {"shortDescription": [{"value": "Wirkung durch Exposition des Menschen mit U235 (IR)", "lang": "de"}, {"value": "Human exposure efficiency relative to U235 (IR)", "lang": "en"}], "type": "LCIA method data set", "refObjectId": "b5c632be-def3-11e6-bf01-fe55135034f3", "uri": "../lciamethods/b5c632be-def3-11e6-bf01-fe55135034f3.xml"}, "other": {"anies": [{"name": "referenceToUnitGroupDataSet", "value": {"shortDescription": [{"value": "kBq U235-Äq.", "lang": "de"}], "type": "unit group data set", "refObjectId": "456b05bf-1415-44a9-9993-02452f554c09", "uri": "../unitgroups/456b05bf-1415-44a9-9993-02452f554c09.xml"}}, {"value": "0.263222258575693", "module": "A1-A3"}, {"value": "0", "module": "C1"}, {"value": "0.0001404725727046", "module": "C2"}, {"value": "0.0459177658226164", "module": "C3"}, {"value": "0", "module": "C4"}, {"value": "-2.58179535993737", "module": "D"}]}}, {"referenceToLCIAMethodDataSet": {"shortDescription": [{"value": "Toxizitätsvergleichseinheit für Ökosysteme (ETP-fw)", "lang": "de"}, {"value": "Comparative toxic unit for ecosystems (ETP-fw)", "lang": "en"}], "type": "LCIA method data set", "refObjectId": "ee1082d1-b0f7-43ca-a1f0-21e2a4a74511", "uri": "../lciamethods/ee1082d1-b0f7-43ca-a1f0-21e2a4a74511.xml"}, "other": {"anies": [{"name": "referenceToUnitGroupDataSet", "value": {"shortDescription": [{"value": "CTUe", "lang": "de"}], "type": "unit group data set", "refObjectId": "aa959ded-f1eb-4efb-9c5c-2d60be36b3e6", "uri": "../unitgroups/aa959ded-f1eb-4efb-9c5c-2d60be36b3e6.xml"}}, {"value": "26.7126564330359", "module": "A1-A3"}, {"value": "0", "module": "C1"}, {"value": "0.353749379748774", "module": "C2"}, {"value": "0.743546194257337", "module": "C3"}, {"value": "0", "module": "C4"}, {"value": "-41.8649286639042", "module": "D"}]}}, {"referenceToLCIAMethodDataSet": {"shortDescription": [{"value": "Toxizitätsvergleichseinheit für Menschen (krebserregend) (HTP-c)", "lang": "de"}, {"value": "Comparative toxic unit for humans (carcinogenic) (HTP-c)", "lang": "en"}], "type": "LCIA method data set", "refObjectId": "2299222a-bbd8-474f-9d4f-4dd1f18aea7c", "uri": "../lciamethods/2299222a-bbd8-474f-9d4f-4dd1f18aea7c.xml"}, "other": {"anies": [{"name": "referenceToUnitGroupDataSet", "value": {"shortDescription": [{"value": "CTUh", "lang": "de"}], "type": "unit group data set", "refObjectId": "d4c9523e-2d7e-49fd-8469-998f547d3a70", "uri": "../unitgroups/d4c9523e-2d7e-49fd-8469-998f547d3a70.xml"}}, {"value": "3.15399427639368E-09", "module": "A1-A3"}, {"value": "0", "module": "C1"}, {"value": "7.29162600877574E-12", "module": "C2"}, {"value": "2.13476872782332E-11", "module": "C3"}, {"value": "0", "module": "C4"}, {"value": "-2.0329982296615E-10", "module": "D"}]}}, {"referenceToLCIAMethodDataSet": {"shortDescription": [{"value": "Toxizitätsvergleichseinheit für Menschen (nicht krebserregend) (HTP-nc)", "lang": "de"}, {"value": "Comparative toxic unit for humans (noncarcinogenic) (HTP-nc)", "lang": "en"}], "type": "LCIA method data set", "refObjectId": "3af763a5-b7a1-48c9-9cee-1f223481fcef", "uri": "../lciamethods/3af763a5-b7a1-48c9-9cee-1f223481fcef.xml"}, "other": {"anies": [{"name": "referenceToUnitGroupDataSet", "value": {"shortDescription": [{"value": "CTUh", "lang": "de"}], "type": "unit group data set", "refObjectId": "d4c9523e-2d7e-49fd-8469-998f547d3a70", "uri": "../unitgroups/d4c9523e-2d7e-49fd-8469-998f547d3a70.xml"}}, {"value": "5.08946840645535E-08", "module": "A1-A3"}, {"value": "0", "module": "C1"}, {"value": "4.46988010044023E-10", "module": "C2"}, {"value": "7.80886771929619E-10", "module": "C3"}, {"value": "0", "module": "C4"}, {"value": "4.74262041671371E-08", "module": "D"}]}}, {"referenceToLCIAMethodDataSet": {"shortDescription": [{"value": "Bodenqualitätsindex (SQP)", "lang": "de"}, {"value": "Soil quality index (SQP)", "lang": "en"}], "type": "LCIA method data set", "refObjectId": "b2ad6890-c78d-11e6-9d9d-cec0c932ce01", "uri": "../lciamethods/b2ad6890-c78d-11e6-9d9d-cec0c932ce01.xml"}, "other": {"anies": [{"name": "referenceToUnitGroupDataSet", "value": {"shortDescription": [{"value": "SQP", "lang": "de"}], "type": "unit group data set", "refObjectId": "f130951c-e67f-4f7f-8dd4-665de3974e18", "uri": "../unitgroups/f130951c-e67f-4f7f-8dd4-665de3974e18.xml"}}, {"value": "566.517748721477", "module": "A1-A3"}, {"value": "0", "module": "C1"}, {"value": "0.21130918783204", "module": "C2"}, {"value": "0.61136535661897", "module": "C3"}, {"value": "0", "module": "C4"}, {"value": "-34.9874114671699", "module": "D"}]}}]}, "otherAttributes": {"{http://www.indata.network/EPD/2019}epd-version": "1.2"}, "version": "1.1", "locations": "../ILCDLocations.xml"}