{"processInformation": {"dataSetInformation": {"UUID": "3dab05f4-58f5-45c5-af52-b3202f127bd7", "name": {"baseName": [{"value": "Drawn Wire – Cold Heading Wire", "lang": "en"}, {"value": "Kaltfließpressdrähte", "lang": "de"}], "functionalUnitFlowProperties": [{"lang": "en"}]}, "classificationInformation": {"classification": [{"class": [{"value": "Metalle", "level": 0, "classId": "4"}, {"value": "Stahl und Eisen", "level": 1, "classId": "4.1"}, {"value": "Stahlprofile", "level": 2, "classId": "4.1.03"}], "name": "OEKOBAU.DAT"}, {"class": [{"value": "02 Building products", "level": 0}, {"value": "Metallic products and ancillaries", "level": 1}, {"value": "Structural steels", "level": 2}], "name": "IBUCategories"}]}, "generalComment": [{"value": "Cold heading wires (CHQ) are used to produce parts of complex shapes by means of cold forming operations, using different production techniques, such as cutting, heading, upsetting, extrusion or rolling. This kind of forming processes can also be complemented by different machining operations, such as turning, grinding, polishing and others.\n\nBearing steel wires are part of the voestalpine Wire Austria GmbH product range. The properties of these wires are optimized to produce ball-, roller-, cylindrical- and needle bearings. Generally, bearing steels are characterized by good hardenability and high surface hardness, which results in little material abrasion during use. \n\nSpring steel wires are also a part of the voestalpine Wire Austria GmbH product range and are used to produce steel springs. Thanks to optimized alloying concepts and processing parameters, spring steel is characterized by its high yield strength to tensile strength ratio, compared to other types of steel. Therefore, spring steels can be subjected to high loads without plastic deformation. \n\nIn order to fulfill certain requirements concerning mechanical properties and deformability, specific chemical compositions, as well as optimized production processes are used to produce cold heading-, bearing steel- and spring steel wires.\nTo ensure high-quality standards, all products are manufactured under optimized process conditions, such as:\n\nHigh degree of purity\nLow core segregation\nOptimized annealing conditions\nContinuous quality inspections and several special testing options\nEnd-to-end traceability of all production and test parameters\nGreatest possible flexibility as the result of an integrated production chain\nStrict adherence to schedules, and partnerships with our customers\nTechnical and sales service", "lang": "en"}, {"value": "Kaltfließpressdrähte (CHQ) werden zur Herstellung von Teilen mit komplexer Form durch Kaltumformung mittels verschiedener Produktionstechniken wie Schneiden, Stauchen, Strangpressen oder Walzen verwendet. Diese Art der Umformung kann auch durch verschiedene Bearbeitungsvorgänge wie Drehen, Schleifen, Polieren und andere ergänzt werden. Lagerstahldrähte sind Teil der Produktpalette der voestalpine Wire Austria GmbH. Die Eigenschaften dieser Drähte sind für die Herstellung von Kugel-, Rollen-, Zylinder- und Nadellagern optimiert. Im Allgemeinen zeichnen sich Lagerstähle durch eine gute Härtbarkeit und hohe Oberflächenhärte aus, was zu einem geringen Materialabrieb während des Gebrauchs führt. \n\nFederstahldrähte sind ebenfalls Teil der Produktpalette der voestalpine Wire Austria GmbH und werden zur Herstellung von Stahlfedern verwendet. Dank optimierter Legierungskonzepte und Verarbeitungsparameter zeichnet sich Federstahl im Vergleich zu anderen Stahlsorten durch ein hohes Verhältnis von Streckgrenze zu Zugfestigkeit aus. Daher können Federstähle hohen Belastungen ausgesetzt werden, ohne sich plastisch zu verformen. \n\nUm bestimmte Anforderungen an die mechanischen Eigenschaften und die Verformbarkeit zu erfüllen, werden für die Herstellung von Kaltstauch-, Wälzlager- und Federstahldrähten spezifische chemische Zusammensetzungen sowie optimierte Produktionsprozesse eingesetzt. Um einen hohen Qualitätsstandard zu gewährleisten, werden alle Produkte unter optimierten Prozessbedingungen hergestellt, wie z.B.: \nHoher Reinheitsgrad \nGeringe Kernseigerung \nOptimierte Glühbedingungen \nStändige Qualitätskontrollen und mehrere spezielle Prüfmöglichkeiten \nDurchgängige Rückverfolgbarkeit aller Produktions- und Prüfparameter \nGrößtmögliche Flexibilität durch eine integrierte Produktionskette \nStrikte Termintreue und Partnerschaft mit unseren Kunden \nTechnischer und vertrieblicher Service", "lang": "de"}]}, "quantitativeReference": {"referenceToReferenceFlow": [0]}, "time": {"referenceYear": 2023, "dataSetValidUntil": 2028, "other": {"anies": [{"name": "publicationDateOfEPD", "value": 1683590400000}]}}, "geography": {"locationOfOperationSupplyOrProduction": {"location": "AT"}}, "technology": {"technologyDescriptionAndIncludedProcesses": [{"value": "The starting material to produce cold heading-, bearing steel- and spring steel wires is low alloyed steel, which is mainly produced at voestalpine Stahl Donawitz GmbH via the primary route (blast furnace, LD steel mill, ladle furnace). The steel is casted into blooms using a continuous casting process. In a further step, the blooms are rolled to the desired dimension in the wire rod rolling mill of voestalpine Wire Rod Austria GmbH. The diameters of the rolled wire rod vary between 5 and 31 mm. After the rolling process the wires are delivered by train to voestalpine Wire Austria GmbH in Bruck an der Mur. In a first step, the wire rods are pickled in hydrochloric acid. At the drawing facility of voestalpine Wire Austria GmbH the wires are further processed according to EN 10263 specifications. The annealing of the coils takes place in a bell-type annealing furnace at temperatures and times of around 700°C and 12 hours. \nTechnical data: \nThis EPD applies to all cold heading-, bearing and spring steel wires from voestalpine Wire Austria GmbH, which is why a general statement about mechanical parameters is not possible. The technical data given for the products are generic literature data for steel as described e.g. in Key to Steel. No product specific test rules are applicable to the data given:\n\nConstructional data\n\nVarious steel grades are processed at the drawing facility of voestalpine Wire Austria GmbH.\n\nCold heading wire steel grades:\n\nFurther steel grades can be processed on request.\n\nBearing wire steel grades:\n\n\nCustomer-specific changes to the alloy composition can occur on request.\n\nSpring wire steel grades:\nSteels according to EN 10270-1 and EN 10089 are used to produce drawn spring steel wire. The following alloys are suitable to produce quenched and tempered springs and are a selection from the voestalpine Wire Austria GmbH product range.\n\n\nCustomer-specific changes to the alloy composition can occur on request. \nDeclared unit: \nThis environmental product declaration refers to a declared unit of 1 tonne of average CHQ-, bearing-, spring steel – automotive wire.", "lang": "en"}, {"value": "Das Ausgangsmaterial für die Herstellung von Kaltfließpress-, Wälzlager- und Federstahldrähten ist niedrig legierter Stahl, der in der voestalpine Stahl Donawitz GmbH hauptsächlich auf dem Primärweg (Hochofen, LD-Stahlwerk, Pfannenofen) hergestellt wird. Der Stahl wird im Stranggussverfahren zu Vorblöcken gegossen.\n\nIn einem weiteren Schritt werden die Vorblöcke im Drahtwalzwerk der voestalpine Wire Rod Austria GmbH auf die gewünschte Abmessung gewalzt. Die Durchmesser des gewalzten Walzdrahtes variieren zwischen 5 und 31 mm. Nach dem Walzprozess werden die Drähte per Bahn an die voestalpine Wire Austria GmbH in Bruck an der Mur geliefert.\n\nIn einem ersten Schritt werden die Walzdrähte in Salzsäure gebeizt. In der Zieherei der voestalpine Wire Austria GmbH werden die Drähte nach den Vorgaben der EN 10263 weiterverarbeitet.\n\nDas Glühen der Coils erfolgt in einem Haubenglühofen bei Temperaturen und Zeiten von etwa 700°C und 12 Stunden. \nTechnische Daten: \nDiese EPD gilt für alle Kaltfließpress-, Lager- und Federstahldrähte der voestalpine Wire Austria GmbH, weshalb eine allgemeine Aussage über mechanische Parameter nicht möglich ist. Die für die Produkte angegebenen technischen Daten sind allgemeine Literaturdaten für Stahl, wie sie z.B. in Stahlschlüssel beschrieben sind. Für die angegebenen Daten gelten keine produktspezifischen Prüfregeln. \nDeklarierte Einheit: \nDiese Umweltproduktdeklaration bezieht sich auf eine deklarierte Einheit von 1 Tonne durchschnittlichen CHQ-, Lager-, Federstahl - Automobildraht.", "lang": "de"}], "technologicalApplicability": [{"value": "Cold heading wire products from voestalpine Wire Austria GmbH are used to produce a variety of components ranging from safety parts, fasteners, fixations, chains, bolts and rivets to ball studs and gear wheels.\n\nSpecial products include cold heading wire for high-strength screws and highly loaded shafts for automotive lightweight construction.\n\nBearing steel wire products from voestalpine Wire Austria GmbH are used in a wide variety of bearing concepts, such as ball-, roller-, cylindrical- or needle bearings.\n\nSpring steel wire products from voestalpine Wire Austria GmbH are characterized by a high yield strength to tensile strength ratio and are therefore well suited to produce a wide variety of spring elements.", "lang": "en"}, {"value": "Kaltfließpressdrahtprodukte der voestalpine Wire Austria GmbH werden zur Herstellung einer Vielzahl von Bauteilen verwendet, wie z.B. von Sicherheitsteilen, Verschlüssen, Befestigungen, Ketten, Bolzen und Nieten bis hin zu Kugelbolzen und Zahnrädern. Zu den Spezialprodukten zählen Kaltstauchdraht für hochfeste Schrauben und hochbelastete Wellen für den automobilen Leichtbau.\n\nLagerstahldrahtprodukte der voestalpine Wire Austria GmbH werden in einer Vielzahl von Lagerkonzepten, wie z.B. Kugel-, Rollen-, Zylinder- oder Nadellagern, eingesetzt. Federstahldrahtprodukte der voestalpine Wire Austria GmbH zeichnen sich durch ein hohes Verhältnis von Streckgrenze zu Zugfestigkeit aus und sind daher für die Herstellung einer Vielzahl von Federelementen gut geeignet.", "lang": "de"}], "referenceToTechnologyFlowDiagrammOrPicture": [{"shortDescription": [{"value": "CHQ Table 1.png", "lang": "en"}], "type": "source data set", "refObjectId": "5d53e5c1-449a-471a-bb88-622b250542a7", "uri": "../sources/5d53e5c1-449a-471a-bb88-622b250542a7.xml"}, {"shortDescription": [{"value": "CHQ Table 2.png", "lang": "en"}], "type": "source data set", "refObjectId": "dda2697d-fcc9-41c9-945c-a093956caf4f", "uri": "../sources/dda2697d-fcc9-41c9-945c-a093956caf4f.xml"}, {"shortDescription": [{"value": "CHQ Table 3.png", "lang": "en"}], "type": "source data set", "refObjectId": "3c51183a-3328-415a-aa33-b1c2b0692b1e", "uri": "../sources/3c51183a-3328-415a-aa33-b1c2b0692b1e.xml"}, {"shortDescription": [{"value": "CHQ Table 4.png", "lang": "en"}], "type": "source data set", "refObjectId": "4c6580af-f736-4727-9c2e-84bf1448cb33", "uri": "../sources/4c6580af-f736-4727-9c2e-84bf1448cb33.xml"}]}}, "modellingAndValidation": {"LCIMethodAndAllocation": {"typeOfDataSet": "EPD", "referenceToLCAMethodDetails": [{"shortDescription": [{"value": "Structural steels.pdf", "lang": "en"}], "type": "source data set", "refObjectId": "4bc01a2b-95a9-4a64-8e2b-c19c315ca055"}], "other": {"anies": [{"name": "subType", "value": "average dataset"}]}}, "dataSourcesTreatmentAndRepresentativeness": {"referenceToDataSource": [{"shortDescription": [{"value": "GaBi Database (all versions)", "lang": "en"}], "type": "source data set", "refObjectId": "28d74cc0-db8b-4d7e-bc44-5f6d56ce0c4a"}, {"shortDescription": [{"value": "GaBi Database Edition 2021, CUP 2021.01", "lang": "en"}], "type": "source data set", "refObjectId": "1cece811-7501-44d4-8067-9259bd5cb835"}], "useAdviceForDataSet": [{"value": "Scope: \nThis EPD is based on a declared unit of 1 metric tonne of average voestalpine cold heading (CHQ)-, bearing-, spring steel wire produced at the production site in Bruck a.d. Mur (Austria). \nSystem boundary: \nThe life cycle assessment of average CHQ-, bearing-, spring steel – automotive wire refers to a cradle-to-gate analysis with modules (A1–A3 + C +D). Subsequent life cycle phases are part of the analysis:\n\nModule A1–A3 | Production stage\nThe production stage includes the burdens of the production of CHQ-, bearing-, spring steel – automotive wire of voestalpine Wire Austria GmbH at the production site in Bruck a.d. Mur. Most of the used steel wire is provided by the voestalpine Wire Rod Austria from St. Peter Freienstein. Thus, the upstream environmental impact of the steel supplied is represented by primary data of the respective production site. Material and energy flows for the pickling, drawing, cold rolling and annealing are considered. Electricity at Bruck a. d. Mur is provided from 100 % renewable energy (emission factor GWP-total: 14 g CO2-equivalents/kWh). Thermal energy provision is based on natural gas. Module A1–A3 also includes the production of the packaging.\n\nModule C1 | Deconstruction and demolition\nIt is assumed that the product is not connected with other materials and can therefore be dismantled. Associated efforts are negligible, no environmental impacts from the deconstruction of the products are declared.\n\nModule C2 | Transport \nThe transport to the disposal of the material is estimated declaring a 50 km radius to the waste processing.\n\nModule C3 | Waste processing \nProduct flows that reach Module D for recycling leave the product system in C3. Environmental impacts resulting from the grinding and sorting of steel scrap are not included due to the negligible expected environmental impact.\n\nModule C4 | Landfilling \nModule C4 declares the environmental impacts incurred by landfilling (5 % of the product).\n\nModule D | Benefits and loads beyond the system boundary\nThe potential for substituting primary steel with a recycling scenario (95 % of the product) is outlined in Module D.", "lang": "en"}, {"value": "Gültigkeitsbereich: \nDiese EPD basiert auf einer deklarierten Einheit von 1 Tonne durchschnittlichen voestalpine Kaltfließpress- (CHQ), Lager-, Federstahldraht, der am Produktionsstandort in Bruck a.d. Mur (Österreich) hergestellt wird. \nSystemgrenze: \nDie Ökobilanz von durchschnittlichem CHQ-, Lager-, Federstahl - Automobildraht bezieht sich auf eine Cradle-to-Gate Analyse mit Modulen (A1-A3 + C +D). Nachfolgende Lebenszyklusphasen sind Teil der Analyse: \n\nModul A1-A3 | Produktionsstadium\nDas Produktionsstadium umfasst die Aufwendungen der Produktion von CHQ-, Lager-, Federstahl - Automobildraht der voestalpine Wire Austria GmbH am Produktionsstandort in Bruck a.d. Mur. Der Großteil des eingesetzten Stahldrahtes wird von der voestalpine Wire Rod Austria aus St. Peter Freienstein geliefert. Die vorgelagerten Umweltauswirkungen des gelieferten Stahls werden daher durch Primärdaten des jeweiligen Produktionsstandortes dargestellt. Die Material- und Energieströme für das Beizen, Ziehen, Kaltwalzen und Glühen werden berücksichtigt. Die Stromversorgung in Bruck a. d. Mur erfolgt zu 100 % aus erneuerbaren Energien (Emissionsfaktor GWP-gesamt: 14 g CO2-Äquivalente/kWh). Die Bereitstellung von thermischer Energie erfolgt auf Basis von Erdgas. Modul A1-A3 umfasst auch die Herstellung der Verpackung. \n\nModul C1 | Rückbau\nFür das End of Life Szenario wird angenommen, dass das Endprodukt nicht mit anderen Materialien verbunden ist und sortenrein rückgebaut werden kann. Die mit dem Rückbau\nverbundenen Aufwände werden damit als gering eingeschätzt und sind somit vernachlässigbar.\n\nModul C2 | Transport \nModul C2 beinhaltet den Transport zur Abfallbehandlung. Dazu wird der Transport via LKW über 50 km Transportdistanz als Szenario angesetzt\n\nModul C3 | Abfallbehandlung \nJener Produktfluss, der das Modul D zum Recycling erreicht, verlässt das Produktsystem in C3. Aufwendungen für die Zerkleinerung und Sortierung des Stahlschrottes sind aufgrund \nder Geringfügigkeit der zu erwartenden Umweltwirkung nicht enthalten.\n\nModul C4 | Entsorgung \nDas Modul C4 deklariert die durch die Deponierung (5 % des Produktes) entstehenden Umweltwirkungen.\n\nModul D | Nutzen und Lasten außerhalb der Systemgrenze \nIm Modul D werden die Substitutionspotenziale von Primärstahl durch ein Recyclingszenario (95 % des Produktes) dargestellt.", "lang": "de"}], "other": {"anies": [{"name": "referenceToOriginalEPD", "value": {"shortDescription": {"value": "Drawn Wire – Cold Heading Wire.pdf", "defaultValue": "Drawn Wire – Cold Heading Wire.pdf", "lstrings": [{"lang": "en", "value": "Drawn Wire – Cold Heading Wire.pdf"}]}, "type": "source data set", "uuid": {"uuid": "dc8b3dba-b2a1-4019-99c1-bafb749bc303"}, "refObjectId": "dc8b3dba-b2a1-4019-99c1-bafb749bc303", "resourceURLs": ["https://oekobaudat.de/OEKOBAU.DAT/resource/sources/dc8b3dba-b2a1-4019-99c1-bafb749bc303/Drawn_Wire_Cold_Heading_Wire_18843.pdf?version=00.03.000"]}}]}}, "validation": {"review": [{"referenceToNameOfReviewerAndInstitution": [{"shortDescription": [{"value": "Institut Bauen und Umwelt e. V.", "lang": "en"}], "type": "contact data set", "refObjectId": "d111dbec-b024-4be5-86c5-752d6eb2cf95", "uri": "../contacts/d111dbec-b024-4be5-86c5-752d6eb2cf95.xml"}], "type": "Accredited third party review"}]}, "complianceDeclarations": {"compliance": [{"referenceToComplianceSystem": {"shortDescription": [{"value": "DIN EN 15804+A2", "lang": "en"}], "type": "source data set", "refObjectId": "c0016b33-8cf7-415c-ac6e-deba0d21440d", "uri": "../sources/c0016b33-8cf7-415c-ac6e-deba0d21440d.xml"}}, {"referenceToComplianceSystem": {"shortDescription": [{"value": "ISO 14025", "lang": "en"}], "type": "source data set", "refObjectId": "4f2eb655-6e44-4874-a95a-e28f5442cd4d", "uri": "../sources/4f2eb655-6e44-4874-a95a-e28f5442cd4d.xml"}}]}}, "administrativeInformation": {"commissionerAndGoal": {"referenceToCommissioner": [{"shortDescription": [{"value": "voestalpine AG", "lang": "en"}], "type": "contact data set", "refObjectId": "eef08a78-bb8b-429e-a968-c40f32a49ec7", "uri": "../contacts/eef08a78-bb8b-429e-a968-c40f32a49ec7.xml"}]}, "dataGenerator": {"referenceToPersonOrEntityGeneratingTheDataSet": [{"shortDescription": [{"value": "Daxner & Merl GmbH", "lang": "en"}], "type": "contact data set", "refObjectId": "ad8ad627-3991-42b7-a7ca-5a3fe0a34c28", "uri": "../contacts/ad8ad627-3991-42b7-a7ca-5a3fe0a34c28.xml"}]}, "dataEntryBy": {"timeStamp": 1683590400000, "referenceToDataSetFormat": [{"shortDescription": [{"value": "ILCD Format", "lang": "en"}], "type": "source data set", "refObjectId": "a97a0155-0234-4b87-b4ce-a45da52f2a40", "uri": "../sources/a97a0155-0234-4b87-b4ce-a45da52f2a40.xml"}, {"shortDescription": [{"value": "EPD-Datenformaterweiterungen v1.2", "lang": "de"}, {"value": "EPD Data Format Extensions v1.2", "lang": "en"}], "type": "source data set", "refObjectId": "a29449fd-aa2f-4de8-b5d7-4b06b43c6fde", "uri": "../sources/a29449fd-aa2f-4de8-b5d7-4b06b43c6fde.xml"}]}, "publicationAndOwnership": {"dataSetVersion": "00.06.000", "referenceToRegistrationAuthority": {"shortDescription": [{"value": "Institut Bauen und Umwelt e. V.", "lang": "en"}], "type": "contact data set", "refObjectId": "d111dbec-b024-4be5-86c5-752d6eb2cf95", "uri": "../contacts/d111dbec-b024-4be5-86c5-752d6eb2cf95.xml"}, "registrationNumber": "EPD-VOE-20230106-IBC2-EN", "referenceToOwnershipOfDataSet": {"shortDescription": [{"value": "voestalpine AG", "lang": "en"}], "type": "contact data set", "refObjectId": "eef08a78-bb8b-429e-a968-c40f32a49ec7", "uri": "../contacts/eef08a78-bb8b-429e-a968-c40f32a49ec7.xml"}, "copyright": true, "licenseType": "Free of charge for all users and uses", "accessRestrictions": [{"value": "None", "lang": "en"}], "other": {"anies": [{"name": "referenceToPublisher", "value": {"shortDescription": [{"value": "Institut Bauen und Umwelt e. V.", "lang": "en"}], "type": "contact data set", "refObjectId": "d111dbec-b024-4be5-86c5-752d6eb2cf95", "uri": "../contacts/d111dbec-b024-4be5-86c5-752d6eb2cf95.xml"}}]}}}, "exchanges": {"exchange": [{"dataSetInternalID": 0, "referenceToFlowDataSet": {"shortDescription": [{"value": "Kaltfließpressdrähte (Kaltfließpressdrähte)", "lang": "en"}], "type": "flow data set", "refObjectId": "6d6e4626-908a-3186-4c59-7335ea3b3d42", "uri": "../flows/6d6e4626-908a-3186-4c59-7335ea3b3d42.xml"}, "meanAmount": 1.0, "referencesToDataSource": {}, "referenceFlow": true, "resolvedFlowVersion": "00.01.000", "resultingflowAmount": 1.0, "flowProperties": [{"name": [{"lang": "en", "value": "Mass"}, {"lang": "de", "value": "Masse"}], "uuid": "93a60a56-a3c8-11da-a746-0800200b9a66", "referenceFlowProperty": true, "meanValue": 1.0, "referenceUnit": "kg", "unitGroupUUID": "ad38d542-3fe9-439d-9b95-2f5f7752acaf"}], "materialProperties": [{"name": "gross density", "value": "7850.0", "unit": "kg/m^3", "unitDescription": "kilograms per cubic metre"}], "typeOfFlow": "Product flow", "classification": {"classHierarchy": "Metalle / Stahl und Eisen / Stahlprofile", "name": "OEKOBAU.DAT"}}, {"dataSetInternalID": 1, "referenceToFlowDataSet": {"shortDescription": [{"value": "Renewable primary energy as energy carrier (PERE)", "lang": "en"}, {"value": "Erneuerbare Primärenergie als Energieträger (PERE)", "lang": "de"}], "type": "flow data set", "refObjectId": "20f32be5-0398-4288-9b6d-accddd195317", "uri": "../flows/20f32be5-0398-4288-9b6d-accddd195317.xml"}, "exchange direction": "INPUT", "other": {"anies": [{"name": "referenceToUnitGroupDataSet", "value": {"shortDescription": [{"value": "MJ", "lang": "en"}], "type": "unit group data set", "refObjectId": "93a60a57-a3c8-11da-a746-0800200c9a66", "uri": "../unitgroups/93a60a57-a3c8-11da-a746-0800200c9a66.xml"}}, {"value": "2149.51332171574", "module": "A1-A3"}, {"value": "0", "module": "C1"}, {"value": "2.29162705358998", "module": "C2"}, {"value": "0", "module": "C3"}, {"value": "2.56802636768431", "module": "C4"}, {"value": "1162.40032793539", "module": "D"}]}, "resolvedFlowVersion": "38.00.000", "flowProperties": [], "typeOfFlow": "Other flow", "classification": {"classHierarchy": "Quantities", "name": "GaBiCategories"}}, {"dataSetInternalID": 2, "referenceToFlowDataSet": {"shortDescription": [{"value": "Renewable primary energy resources as material utilization (PERM)", "lang": "en"}, {"value": "Erneuerbare Primärenergie zur stofflichen Nutzung (PERM)", "lang": "de"}], "type": "flow data set", "refObjectId": "fb3ec0de-548d-4508-aea5-00b73bf6f702", "uri": "../flows/fb3ec0de-548d-4508-aea5-00b73bf6f702.xml"}, "exchange direction": "INPUT", "other": {"anies": [{"name": "referenceToUnitGroupDataSet", "value": {"shortDescription": [{"value": "MJ", "lang": "en"}], "type": "unit group data set", "refObjectId": "93a60a57-a3c8-11da-a746-0800200c9a66", "uri": "../unitgroups/93a60a57-a3c8-11da-a746-0800200c9a66.xml"}}, {"value": "138.847974828321", "module": "A1-A3"}, {"value": "0", "module": "C1"}, {"value": "0", "module": "C2"}, {"value": "0", "module": "C3"}, {"value": "0", "module": "C4"}, {"value": "0", "module": "D"}]}, "resolvedFlowVersion": "38.00.000", "flowProperties": [], "typeOfFlow": "Other flow", "classification": {"classHierarchy": "Quantities", "name": "GaBiCategories"}}, {"dataSetInternalID": 3, "referenceToFlowDataSet": {"shortDescription": [{"value": "Total use of renewable primary energy resources (PERT)", "lang": "en"}, {"value": "Total erneuerbare Primärenergie (PERT)", "lang": "de"}], "type": "flow data set", "refObjectId": "53f97275-fa8a-4cdd-9024-65936002acd0", "uri": "../flows/53f97275-fa8a-4cdd-9024-65936002acd0.xml"}, "exchange direction": "INPUT", "other": {"anies": [{"name": "referenceToUnitGroupDataSet", "value": {"shortDescription": [{"value": "MJ", "lang": "en"}], "type": "unit group data set", "refObjectId": "93a60a57-a3c8-11da-a746-0800200c9a66", "uri": "../unitgroups/93a60a57-a3c8-11da-a746-0800200c9a66.xml"}}, {"value": "2288.36129654406", "module": "A1-A3"}, {"value": "0", "module": "C1"}, {"value": "2.29162705358998", "module": "C2"}, {"value": "0", "module": "C3"}, {"value": "2.56802636768431", "module": "C4"}, {"value": "1162.40032793539", "module": "D"}]}, "resolvedFlowVersion": "38.00.000", "flowProperties": [], "typeOfFlow": "Other flow", "classification": {"classHierarchy": "Quantities / Environmental quantities / EPD EN 15804 / LCI indicators", "name": "GaBiCategories"}}, {"dataSetInternalID": 4, "referenceToFlowDataSet": {"shortDescription": [{"value": "Non renewable primary energy as energy carrier (PENRE)", "lang": "en"}, {"value": "Nicht-erneuerbare Primärenergie als Energieträger (PENRE)", "lang": "de"}], "type": "flow data set", "refObjectId": "ac857178-2b45-46ec-892a-a9a4332f0372", "uri": "../flows/ac857178-2b45-46ec-892a-a9a4332f0372.xml"}, "exchange direction": "INPUT", "other": {"anies": [{"name": "referenceToUnitGroupDataSet", "value": {"shortDescription": [{"value": "MJ", "lang": "en"}], "type": "unit group data set", "refObjectId": "93a60a57-a3c8-11da-a746-0800200c9a66", "uri": "../unitgroups/93a60a57-a3c8-11da-a746-0800200c9a66.xml"}}, {"value": "26849.3168379642", "module": "A1-A3"}, {"value": "0", "module": "C1"}, {"value": "39.9699776934577", "module": "C2"}, {"value": "0", "module": "C3"}, {"value": "35.560110058703", "module": "C4"}, {"value": "-12642.6016689934", "module": "D"}]}, "resolvedFlowVersion": "38.00.000", "flowProperties": [], "typeOfFlow": "Other flow", "classification": {"classHierarchy": "Quantities", "name": "GaBiCategories"}}, {"dataSetInternalID": 5, "referenceToFlowDataSet": {"shortDescription": [{"value": "Non renewable primary energy as material utilization (PENRM)", "lang": "en"}, {"value": "Nicht-erneuerbare Primärenergie zur stofflichen Nutzung (PENRM)", "lang": "de"}], "type": "flow data set", "refObjectId": "1421caa0-679d-4bf4-b282-0eb850ccae27", "uri": "../flows/1421caa0-679d-4bf4-b282-0eb850ccae27.xml"}, "exchange direction": "INPUT", "other": {"anies": [{"name": "referenceToUnitGroupDataSet", "value": {"shortDescription": [{"value": "MJ", "lang": "en"}], "type": "unit group data set", "refObjectId": "93a60a57-a3c8-11da-a746-0800200c9a66", "uri": "../unitgroups/93a60a57-a3c8-11da-a746-0800200c9a66.xml"}}, {"value": "5.684908086", "module": "A1-A3"}, {"value": "0", "module": "C1"}, {"value": "0", "module": "C2"}, {"value": "0", "module": "C3"}, {"value": "0", "module": "C4"}, {"value": "0", "module": "D"}]}, "resolvedFlowVersion": "38.00.000", "flowProperties": [], "typeOfFlow": "Other flow", "classification": {"classHierarchy": "Quantities", "name": "GaBiCategories"}}, {"dataSetInternalID": 6, "referenceToFlowDataSet": {"shortDescription": [{"value": "Total use of non renewable primary energy resources (PENRT)", "lang": "en"}, {"value": "Total nicht erneuerbare Primärenergie (PENRT)", "lang": "de"}], "type": "flow data set", "refObjectId": "06159210-646b-4c8d-8583-da9b3b95a6c1", "uri": "../flows/06159210-646b-4c8d-8583-da9b3b95a6c1.xml"}, "exchange direction": "INPUT", "other": {"anies": [{"name": "referenceToUnitGroupDataSet", "value": {"shortDescription": [{"value": "MJ", "lang": "en"}], "type": "unit group data set", "refObjectId": "93a60a57-a3c8-11da-a746-0800200c9a66", "uri": "../unitgroups/93a60a57-a3c8-11da-a746-0800200c9a66.xml"}}, {"value": "26855.0017460502", "module": "A1-A3"}, {"value": "0", "module": "C1"}, {"value": "39.9699776934577", "module": "C2"}, {"value": "0", "module": "C3"}, {"value": "35.560110058703", "module": "C4"}, {"value": "-12642.6016689934", "module": "D"}]}, "resolvedFlowVersion": "38.00.000", "flowProperties": [], "typeOfFlow": "Other flow", "classification": {"classHierarchy": "Quantities / Environmental quantities / EPD EN 15804 / LCI indicators", "name": "GaBiCategories"}}, {"dataSetInternalID": 7, "referenceToFlowDataSet": {"shortDescription": [{"value": "Use of secondary material (SM)", "lang": "en"}, {"value": "Einsatz von Sekundärstoffen (SM)", "lang": "de"}], "type": "flow data set", "refObjectId": "c6a1f35f-2d09-4f54-8dfb-97e502e1ce92", "uri": "../flows/c6a1f35f-2d09-4f54-8dfb-97e502e1ce92.xml"}, "exchange direction": "INPUT", "other": {"anies": [{"name": "referenceToUnitGroupDataSet", "value": {"shortDescription": [{"value": "kg", "lang": "en"}], "type": "unit group data set", "refObjectId": "ad38d542-3fe9-439d-9b95-2f5f7752acaf", "uri": "../unitgroups/ad38d542-3fe9-439d-9b95-2f5f7752acaf.xml"}}, {"value": "115.611", "module": "A1-A3"}, {"value": "0", "module": "C1"}, {"value": "0", "module": "C2"}, {"value": "0", "module": "C3"}, {"value": "0", "module": "C4"}, {"value": "856.425", "module": "D"}]}, "resolvedFlowVersion": "38.00.000", "flowProperties": [], "typeOfFlow": "Other flow", "classification": {"classHierarchy": "Quantities / Environmental quantities / EPD EN 15804 / LCI indicators", "name": "GaBiCategories"}}, {"dataSetInternalID": 8, "referenceToFlowDataSet": {"shortDescription": [{"value": "Use of renewable secondary fuels (RSF)", "lang": "en"}, {"value": "Erneuerbare Sekundärbrennstoffe (RSF)", "lang": "de"}], "type": "flow data set", "refObjectId": "64333088-a55f-4aa2-9a31-c10b07816787", "uri": "../flows/64333088-a55f-4aa2-9a31-c10b07816787.xml"}, "exchange direction": "INPUT", "other": {"anies": [{"name": "referenceToUnitGroupDataSet", "value": {"shortDescription": [{"value": "MJ", "lang": "en"}], "type": "unit group data set", "refObjectId": "93a60a57-a3c8-11da-a746-0800200c9a66", "uri": "../unitgroups/93a60a57-a3c8-11da-a746-0800200c9a66.xml"}}, {"value": "0", "module": "A1-A3"}, {"value": "0", "module": "C1"}, {"value": "0", "module": "C2"}, {"value": "0", "module": "C3"}, {"value": "0", "module": "C4"}, {"value": "0", "module": "D"}]}, "resolvedFlowVersion": "38.00.000", "flowProperties": [], "typeOfFlow": "Other flow", "classification": {"classHierarchy": "Quantities / Environmental quantities / EPD EN 15804 / LCI indicators", "name": "GaBiCategories"}}, {"dataSetInternalID": 9, "referenceToFlowDataSet": {"shortDescription": [{"value": "Use of non renewable secondary fuels (NRSF)", "lang": "en"}, {"value": "Nicht erneuerbare Sekundärbrennstoffe (NRSF)", "lang": "de"}], "type": "flow data set", "refObjectId": "89def144-d39a-4287-b86f-efde453ddcb2", "uri": "../flows/89def144-d39a-4287-b86f-efde453ddcb2.xml"}, "exchange direction": "INPUT", "other": {"anies": [{"name": "referenceToUnitGroupDataSet", "value": {"shortDescription": [{"value": "MJ", "lang": "en"}], "type": "unit group data set", "refObjectId": "93a60a57-a3c8-11da-a746-0800200c9a66", "uri": "../unitgroups/93a60a57-a3c8-11da-a746-0800200c9a66.xml"}}, {"value": "0", "module": "A1-A3"}, {"value": "0", "module": "C1"}, {"value": "0", "module": "C2"}, {"value": "0", "module": "C3"}, {"value": "0", "module": "C4"}, {"value": "0", "module": "D"}]}, "resolvedFlowVersion": "38.00.000", "flowProperties": [], "typeOfFlow": "Other flow", "classification": {"classHierarchy": "Quantities / Environmental quantities / EPD EN 15804 / LCI indicators", "name": "GaBiCategories"}}, {"dataSetInternalID": 10, "referenceToFlowDataSet": {"shortDescription": [{"value": "Use of net fresh water (FW)", "lang": "en"}, {"value": "Einsatz von Süßwasserressourcen (FW)", "lang": "de"}], "type": "flow data set", "refObjectId": "3cf952c8-f3a4-461d-8c96-96456ca62246", "uri": "../flows/3cf952c8-f3a4-461d-8c96-96456ca62246.xml"}, "exchange direction": "INPUT", "other": {"anies": [{"name": "referenceToUnitGroupDataSet", "value": {"shortDescription": [{"value": "m^3", "lang": "en"}], "type": "unit group data set", "refObjectId": "cd950537-0a98-4044-9ba7-9f9a68d0a504", "uri": "../unitgroups/cd950537-0a98-4044-9ba7-9f9a68d0a504.xml"}}, {"value": "15.0319587138865", "module": "A1-A3"}, {"value": "0", "module": "C1"}, {"value": "0.00262465508256471", "module": "C2"}, {"value": "0", "module": "C3"}, {"value": "0.000367450889833254", "module": "C4"}, {"value": "-6.39919490250304", "module": "D"}]}, "resolvedFlowVersion": "38.00.000", "flowProperties": [], "typeOfFlow": "Other flow", "classification": {"classHierarchy": "Quantities / Environmental quantities / EPD EN 15804 / LCI indicators", "name": "GaBiCategories"}}, {"dataSetInternalID": 11, "referenceToFlowDataSet": {"shortDescription": [{"value": "Hazardous waste disposed (HWD)", "lang": "en"}, {"value": "Gefährlicher Abfall zur Deponie (HWD)", "lang": "de"}], "type": "flow data set", "refObjectId": "430f9e0f-59b2-46a0-8e0d-55e0e84948fc", "uri": "../flows/430f9e0f-59b2-46a0-8e0d-55e0e84948fc.xml"}, "exchange direction": "OUTPUT", "other": {"anies": [{"name": "referenceToUnitGroupDataSet", "value": {"shortDescription": [{"value": "kg", "lang": "en"}], "type": "unit group data set", "refObjectId": "ad38d542-3fe9-439d-9b95-2f5f7752acaf", "uri": "../unitgroups/ad38d542-3fe9-439d-9b95-2f5f7752acaf.xml"}}, {"value": "7.9215490676384E-06", "module": "A1-A3"}, {"value": "0", "module": "C1"}, {"value": "2.10610417494668E-09", "module": "C2"}, {"value": "0", "module": "C3"}, {"value": "6.30055255131535E-09", "module": "C4"}, {"value": "3.52534478177622E-06", "module": "D"}]}, "resolvedFlowVersion": "38.00.000", "flowProperties": [], "typeOfFlow": "Other flow", "classification": {"classHierarchy": "Quantities / Environmental quantities / EPD EN 15804 / LCI indicators", "name": "GaBiCategories"}}, {"dataSetInternalID": 12, "referenceToFlowDataSet": {"shortDescription": [{"value": "Non hazardous waste disposed (NHWD)", "lang": "en"}, {"value": "Entsorgter nicht gefährlicher Abfall (NHWD)", "lang": "de"}], "type": "flow data set", "refObjectId": "b29ef66b-e286-4afa-949f-62f1a7b4d7fa", "uri": "../flows/b29ef66b-e286-4afa-949f-62f1a7b4d7fa.xml"}, "exchange direction": "OUTPUT", "other": {"anies": [{"name": "referenceToUnitGroupDataSet", "value": {"shortDescription": [{"value": "kg", "lang": "en"}], "type": "unit group data set", "refObjectId": "ad38d542-3fe9-439d-9b95-2f5f7752acaf", "uri": "../unitgroups/ad38d542-3fe9-439d-9b95-2f5f7752acaf.xml"}}, {"value": "70.6600105119193", "module": "A1-A3"}, {"value": "0", "module": "C1"}, {"value": "0.006270810990958", "module": "C2"}, {"value": "0", "module": "C3"}, {"value": "50.0681660982345", "module": "C4"}, {"value": "151.970328949715", "module": "D"}]}, "resolvedFlowVersion": "38.00.000", "flowProperties": [], "typeOfFlow": "Other flow", "classification": {"classHierarchy": "Quantities / Environmental quantities / EPD EN 15804 / LCI indicators", "name": "GaBiCategories"}}, {"dataSetInternalID": 13, "referenceToFlowDataSet": {"shortDescription": [{"value": "Radioactive waste disposed (RWD)", "lang": "en"}, {"value": "Entsorgter radioaktiver Abfall (RWD)", "lang": "de"}], "type": "flow data set", "refObjectId": "3449546e-52ad-4b39-b809-9fb77cea8ff6", "uri": "../flows/3449546e-52ad-4b39-b809-9fb77cea8ff6.xml"}, "exchange direction": "OUTPUT", "other": {"anies": [{"name": "referenceToUnitGroupDataSet", "value": {"shortDescription": [{"value": "kg", "lang": "en"}], "type": "unit group data set", "refObjectId": "ad38d542-3fe9-439d-9b95-2f5f7752acaf", "uri": "../unitgroups/ad38d542-3fe9-439d-9b95-2f5f7752acaf.xml"}}, {"value": "0.135224166568212", "module": "A1-A3"}, {"value": "0", "module": "C1"}, {"value": "7.25025813208313E-05", "module": "C2"}, {"value": "0", "module": "C3"}, {"value": "0.00040531725055476", "module": "C4"}, {"value": "0.00045760903856233", "module": "D"}]}, "resolvedFlowVersion": "38.00.000", "flowProperties": [], "typeOfFlow": "Other flow", "classification": {"classHierarchy": "Quantities / Environmental quantities / EPD EN 15804 / LCI indicators", "name": "GaBiCategories"}}, {"dataSetInternalID": 14, "referenceToFlowDataSet": {"shortDescription": [{"value": "Components for re-use (CRU)", "lang": "en"}, {"value": "Komponenten für die Wiederverwendung (CRU)", "lang": "de"}], "type": "flow data set", "refObjectId": "a2b32f97-3fc7-4af2-b209-525bc6426f33", "uri": "../flows/a2b32f97-3fc7-4af2-b209-525bc6426f33.xml"}, "exchange direction": "OUTPUT", "other": {"anies": [{"name": "referenceToUnitGroupDataSet", "value": {"shortDescription": [{"value": "kg", "lang": "en"}], "type": "unit group data set", "refObjectId": "ad38d542-3fe9-439d-9b95-2f5f7752acaf", "uri": "../unitgroups/ad38d542-3fe9-439d-9b95-2f5f7752acaf.xml"}}, {"value": "0", "module": "A1-A3"}, {"value": "0", "module": "C1"}, {"value": "0", "module": "C2"}, {"value": "0", "module": "C3"}, {"value": "0", "module": "C4"}, {"value": "0", "module": "D"}]}, "resolvedFlowVersion": "38.00.000", "flowProperties": [], "typeOfFlow": "Other flow", "classification": {"classHierarchy": "Quantities / Environmental quantities / EPD EN 15804 / LCI indicators", "name": "GaBiCategories"}}, {"dataSetInternalID": 15, "referenceToFlowDataSet": {"shortDescription": [{"value": "Materials for recycling (MFR)", "lang": "en"}, {"value": "Stoffe zum Recycling (MFR)", "lang": "de"}], "type": "flow data set", "refObjectId": "d7fe48a5-4103-49c8-9aae-b0b5dfdbd6ae", "uri": "../flows/d7fe48a5-4103-49c8-9aae-b0b5dfdbd6ae.xml"}, "exchange direction": "OUTPUT", "other": {"anies": [{"name": "referenceToUnitGroupDataSet", "value": {"shortDescription": [{"value": "kg", "lang": "en"}], "type": "unit group data set", "refObjectId": "ad38d542-3fe9-439d-9b95-2f5f7752acaf", "uri": "../unitgroups/ad38d542-3fe9-439d-9b95-2f5f7752acaf.xml"}}, {"value": "0", "module": "A1-A3"}, {"value": "0", "module": "C1"}, {"value": "0", "module": "C2"}, {"value": "950", "module": "C3"}, {"value": "0", "module": "C4"}, {"value": "0", "module": "D"}]}, "resolvedFlowVersion": "38.00.000", "flowProperties": [], "typeOfFlow": "Other flow", "classification": {"classHierarchy": "Quantities / Environmental quantities / EPD EN 15804 / LCI indicators", "name": "GaBiCategories"}}, {"dataSetInternalID": 16, "referenceToFlowDataSet": {"shortDescription": [{"value": "Materials for energy recovery (MER)", "lang": "en"}, {"value": "Stoffe für die Energierückgewinnung (MER)", "lang": "de"}], "type": "flow data set", "refObjectId": "59a9181c-3aaf-46ee-8b13-2b3723b6e447", "uri": "../flows/59a9181c-3aaf-46ee-8b13-2b3723b6e447.xml"}, "exchange direction": "OUTPUT", "other": {"anies": [{"name": "referenceToUnitGroupDataSet", "value": {"shortDescription": [{"value": "kg", "lang": "en"}], "type": "unit group data set", "refObjectId": "ad38d542-3fe9-439d-9b95-2f5f7752acaf", "uri": "../unitgroups/ad38d542-3fe9-439d-9b95-2f5f7752acaf.xml"}}, {"value": "0", "module": "A1-A3"}, {"value": "0", "module": "C1"}, {"value": "0", "module": "C2"}, {"value": "0", "module": "C3"}, {"value": "0", "module": "C4"}, {"value": "0", "module": "D"}]}, "resolvedFlowVersion": "38.00.000", "flowProperties": [], "typeOfFlow": "Other flow", "classification": {"classHierarchy": "Quantities / Environmental quantities / EPD EN 15804 / LCI indicators", "name": "GaBiCategories"}}, {"dataSetInternalID": 17, "referenceToFlowDataSet": {"shortDescription": [{"value": "Exported electrical energy (EEE)", "lang": "en"}, {"value": "Exportierte elektrische Energie (EEE)", "lang": "de"}], "type": "flow data set", "refObjectId": "4da0c987-2b76-40d6-9e9e-82a017aaaf29", "uri": "../flows/4da0c987-2b76-40d6-9e9e-82a017aaaf29.xml"}, "exchange direction": "OUTPUT", "other": {"anies": [{"name": "referenceToUnitGroupDataSet", "value": {"shortDescription": [{"value": "MJ", "lang": "en"}], "type": "unit group data set", "refObjectId": "93a60a57-a3c8-11da-a746-0800200c9a66", "uri": "../unitgroups/93a60a57-a3c8-11da-a746-0800200c9a66.xml"}}, {"value": "0", "module": "A1-A3"}, {"value": "0", "module": "C1"}, {"value": "0", "module": "C2"}, {"value": "0", "module": "C3"}, {"value": "0", "module": "C4"}, {"value": "0", "module": "D"}]}, "resolvedFlowVersion": "38.00.000", "flowProperties": [], "typeOfFlow": "Other flow", "classification": {"classHierarchy": "Quantities / Environmental quantities / EPD EN 15804 / LCI indicators", "name": "GaBiCategories"}}, {"dataSetInternalID": 18, "referenceToFlowDataSet": {"shortDescription": [{"value": "Exported thermal energy (EET)", "lang": "en"}, {"value": "Exportierte thermische Energie (EET)", "lang": "de"}], "type": "flow data set", "refObjectId": "98daf38a-7a79-46d3-9a37-2b7bd0955810", "uri": "../flows/98daf38a-7a79-46d3-9a37-2b7bd0955810.xml"}, "exchange direction": "OUTPUT", "other": {"anies": [{"name": "referenceToUnitGroupDataSet", "value": {"shortDescription": [{"value": "MJ", "lang": "en"}], "type": "unit group data set", "refObjectId": "93a60a57-a3c8-11da-a746-0800200c9a66", "uri": "../unitgroups/93a60a57-a3c8-11da-a746-0800200c9a66.xml"}}, {"value": "0", "module": "A1-A3"}, {"value": "0", "module": "C1"}, {"value": "0", "module": "C2"}, {"value": "0", "module": "C3"}, {"value": "0", "module": "C4"}, {"value": "0", "module": "D"}]}, "resolvedFlowVersion": "38.00.000", "flowProperties": [], "typeOfFlow": "Other flow", "classification": {"classHierarchy": "Quantities / Environmental quantities / EPD EN 15804 / LCI indicators", "name": "GaBiCategories"}}]}, "LCIAResults": {"LCIAResult": [{"referenceToLCIAMethodDataSet": {"shortDescription": [{"value": "Global Warming Potential total (GWP-total)", "lang": "en"}, {"value": "Globales Erwärmungspotenzial total (GWP-total)", "lang": "de"}], "type": "LCIA method data set", "refObjectId": "6a37f984-a4b3-458a-a20a-64418c145fa2", "uri": "../lciamethods/6a37f984-a4b3-458a-a20a-64418c145fa2.xml"}, "other": {"anies": [{"name": "referenceToUnitGroupDataSet", "value": {"shortDescription": [{"value": "kg CO_(2) eq", "lang": "en"}], "type": "unit group data set", "refObjectId": "1ebf3012-d0db-4de2-aefd-ef30cedb0be1", "uri": "../unitgroups/1ebf3012-d0db-4de2-aefd-ef30cedb0be1.xml"}}, {"value": "2926.1594517994", "module": "A1-A3"}, {"value": "0", "module": "C1"}, {"value": "3.02406984359964", "module": "C2"}, {"value": "0", "module": "C3"}, {"value": "2.41918382472411", "module": "C4"}, {"value": "-1452.79737605603", "module": "D"}]}}, {"referenceToLCIAMethodDataSet": {"shortDescription": [{"value": "Global Warming Potential fossil fuels (GWP-fossil)", "lang": "en"}, {"value": "Globales Erwärmungspotenzial fossil (GWP-fossil)", "lang": "de"}], "type": "LCIA method data set", "refObjectId": "5f635281-343e-44fb-83df-1971b155e6b6", "uri": "../lciamethods/5f635281-343e-44fb-83df-1971b155e6b6.xml"}, "other": {"anies": [{"name": "referenceToUnitGroupDataSet", "value": {"shortDescription": [{"value": "kg CO_(2) eq", "lang": "en"}], "type": "unit group data set", "refObjectId": "1ebf3012-d0db-4de2-aefd-ef30cedb0be1", "uri": "../unitgroups/1ebf3012-d0db-4de2-aefd-ef30cedb0be1.xml"}}, {"value": "2904.20817804574", "module": "A1-A3"}, {"value": "0", "module": "C1"}, {"value": "3.00319194896064", "module": "C2"}, {"value": "0", "module": "C3"}, {"value": "2.44174990564248", "module": "C4"}, {"value": "-1452.06685022933", "module": "D"}]}}, {"referenceToLCIAMethodDataSet": {"shortDescription": [{"value": "Global Warming Potential biogenic (GWP-biogenic)", "lang": "en"}, {"value": "Globales Erwärmungspotenzial biogen (GWP-biogenic)", "lang": "de"}], "type": "LCIA method data set", "refObjectId": "2356e1ab-0185-4db5-86e5-16de51c7485c", "uri": "../lciamethods/2356e1ab-0185-4db5-86e5-16de51c7485c.xml"}, "other": {"anies": [{"name": "referenceToUnitGroupDataSet", "value": {"shortDescription": [{"value": "kg CO_(2) eq", "lang": "en"}], "type": "unit group data set", "refObjectId": "1ebf3012-d0db-4de2-aefd-ef30cedb0be1", "uri": "../unitgroups/1ebf3012-d0db-4de2-aefd-ef30cedb0be1.xml"}}, {"value": "20.9493283923947", "module": "A1-A3"}, {"value": "0", "module": "C1"}, {"value": "-0.00356121612494437", "module": "C2"}, {"value": "0", "module": "C3"}, {"value": "-0.0250097349651544", "module": "C4"}, {"value": "-0.940671212982575", "module": "D"}]}}, {"referenceToLCIAMethodDataSet": {"shortDescription": [{"value": "Global Warming Potential luluc (GWP-luluc)", "lang": "en"}, {"value": "Globales Erwärmungspotenzial luluc (GWP-luluc)", "lang": "de"}], "type": "LCIA method data set", "refObjectId": "4331bbdb-978a-490d-8707-eeb047f01a55", "uri": "../lciamethods/4331bbdb-978a-490d-8707-eeb047f01a55.xml"}, "other": {"anies": [{"name": "referenceToUnitGroupDataSet", "value": {"shortDescription": [{"value": "kg CO_(2) eq", "lang": "en"}], "type": "unit group data set", "refObjectId": "1ebf3012-d0db-4de2-aefd-ef30cedb0be1", "uri": "../unitgroups/1ebf3012-d0db-4de2-aefd-ef30cedb0be1.xml"}}, {"value": "1.00194536126574", "module": "A1-A3"}, {"value": "0", "module": "C1"}, {"value": "0.0244391107639501", "module": "C2"}, {"value": "0", "module": "C3"}, {"value": "0.0024436540467793", "module": "C4"}, {"value": "0.210145386275992", "module": "D"}]}}, {"referenceToLCIAMethodDataSet": {"shortDescription": [{"value": "Depletion potential of the stratospheric ozone layer (ODP)", "lang": "en"}, {"value": "Abbau Potential der stratosphärischen Ozonschicht (ODP)", "lang": "de"}], "type": "LCIA method data set", "refObjectId": "b5c629d6-def3-11e6-bf01-fe55135034f3", "uri": "../lciamethods/b5c629d6-def3-11e6-bf01-fe55135034f3.xml"}, "other": {"anies": [{"name": "referenceToUnitGroupDataSet", "value": {"shortDescription": [{"value": "kg CFC11 eq", "lang": "en"}], "type": "unit group data set", "refObjectId": "d9e957c9-7309-4474-bf3a-7777df6c4e5b", "uri": "../unitgroups/d9e957c9-7309-4474-bf3a-7777df6c4e5b.xml"}}, {"value": "8.57475201689271E-12", "module": "A1-A3"}, {"value": "0", "module": "C1"}, {"value": "5.90297134895215E-16", "module": "C2"}, {"value": "0", "module": "C3"}, {"value": "5.76801483752193E-15", "module": "C4"}, {"value": "-2.42111387696885E-12", "module": "D"}]}}, {"referenceToLCIAMethodDataSet": {"shortDescription": [{"value": "Acidification potential of land and water (AP)", "lang": "en"}, {"value": "Versauerungspotenzial von Boden und Wasser (AP)", "lang": "de"}], "type": "LCIA method data set", "refObjectId": "b5c611c6-def3-11e6-bf01-fe55135034f3", "uri": "../lciamethods/b5c611c6-def3-11e6-bf01-fe55135034f3.xml"}, "other": {"anies": [{"name": "referenceToUnitGroupDataSet", "value": {"shortDescription": [{"value": "mol H^(+) eq", "lang": "en"}], "type": "unit group data set", "refObjectId": "42e089ac-92bf-4bf2-8ca1-5fc40d18f2ed", "uri": "../unitgroups/42e089ac-92bf-4bf2-8ca1-5fc40d18f2ed.xml"}}, {"value": "8.9888157962522", "module": "A1-A3"}, {"value": "0", "module": "C1"}, {"value": "0.00991631767120497", "module": "C2"}, {"value": "0", "module": "C3"}, {"value": "0.00777562069923066", "module": "C4"}, {"value": "-2.60661242098874", "module": "D"}]}}, {"referenceToLCIAMethodDataSet": {"shortDescription": [{"value": "Eutrophication potential aquatic freshwater (EP-freshwater)", "lang": "en"}, {"value": "Eutrophierungspotenzial Süßwasser (EP-freshwater)", "lang": "de"}], "type": "LCIA method data set", "refObjectId": "b53ec18f-7377-4ad3-86eb-cc3f4f276b2b", "uri": "../lciamethods/b53ec18f-7377-4ad3-86eb-cc3f4f276b2b.xml"}, "other": {"anies": [{"name": "referenceToUnitGroupDataSet", "value": {"shortDescription": [{"value": "kg P eq", "lang": "en"}], "type": "unit group data set", "refObjectId": "0429039d-a61d-4590-ba67-aa4a20a810a1", "uri": "../unitgroups/0429039d-a61d-4590-ba67-aa4a20a810a1.xml"}}, {"value": "0.0161924795581248", "module": "A1-A3"}, {"value": "0", "module": "C1"}, {"value": "8.88275548806866E-06", "module": "C2"}, {"value": "0", "module": "C3"}, {"value": "1.8584714056159E-06", "module": "C4"}, {"value": "-0.000296923278869942", "module": "D"}]}}, {"referenceToLCIAMethodDataSet": {"shortDescription": [{"value": "Eutrophication potential aquatic marine (EP-marine)", "lang": "en"}, {"value": "Eutrophierungspotenzial Salzwasser (EP-marine)", "lang": "de"}], "type": "LCIA method data set", "refObjectId": "b5c619fa-def3-11e6-bf01-fe55135034f3", "uri": "../lciamethods/b5c619fa-def3-11e6-bf01-fe55135034f3.xml"}, "other": {"anies": [{"name": "referenceToUnitGroupDataSet", "value": {"shortDescription": [{"value": "kg N eq", "lang": "en"}], "type": "unit group data set", "refObjectId": "d05bb823-ecdf-4686-8c40-bf1d9257859f", "uri": "../unitgroups/d05bb823-ecdf-4686-8c40-bf1d9257859f.xml"}}, {"value": "2.1674971927135", "module": "A1-A3"}, {"value": "0", "module": "C1"}, {"value": "0.004554984082094", "module": "C2"}, {"value": "0", "module": "C3"}, {"value": "0.00193046056746469", "module": "C4"}, {"value": "-0.38846960498727", "module": "D"}]}}, {"referenceToLCIAMethodDataSet": {"shortDescription": [{"value": "Eutrophication potential terrestrial (EP-terrestrial)", "lang": "en"}, {"value": "Eutrophierungspotenzial Land (EP-terrestrial)", "lang": "de"}], "type": "LCIA method data set", "refObjectId": "b5c614d2-def3-11e6-bf01-fe55135034f3", "uri": "../lciamethods/b5c614d2-def3-11e6-bf01-fe55135034f3.xml"}, "other": {"anies": [{"name": "referenceToUnitGroupDataSet", "value": {"shortDescription": [{"value": "mol N eq", "lang": "en"}], "type": "unit group data set", "refObjectId": "71b4d617-0ec9-4d3f-b65e-e438940c2401", "uri": "../unitgroups/71b4d617-0ec9-4d3f-b65e-e438940c2401.xml"}}, {"value": "23.1221251655391", "module": "A1-A3"}, {"value": "0", "module": "C1"}, {"value": "0.0508448603038948", "module": "C2"}, {"value": "0", "module": "C3"}, {"value": "0.0211802245417931", "module": "C4"}, {"value": "-3.78722019221668", "module": "D"}]}}, {"referenceToLCIAMethodDataSet": {"shortDescription": [{"value": "Formation potential of tropospheric ozone photochemical oxidants (POCP)", "lang": "en"}, {"value": "Bildungspotential für troposphärisches Ozon (POCP)", "lang": "de"}], "type": "LCIA method data set", "refObjectId": "b5c610fe-def3-11e6-bf01-fe55135034f3", "uri": "../lciamethods/b5c610fe-def3-11e6-bf01-fe55135034f3.xml"}, "other": {"anies": [{"name": "referenceToUnitGroupDataSet", "value": {"shortDescription": [{"value": "kg NMVOC eq", "lang": "en"}], "type": "unit group data set", "refObjectId": "d27c25f8-fbc1-44c6-b47b-4adbae4199c6", "uri": "../unitgroups/d27c25f8-fbc1-44c6-b47b-4adbae4199c6.xml"}}, {"value": "7.24103641702456", "module": "A1-A3"}, {"value": "0", "module": "C1"}, {"value": "0.0089410805422895", "module": "C2"}, {"value": "0", "module": "C3"}, {"value": "0.00608284454471822", "module": "C4"}, {"value": "-1.9888274863866", "module": "D"}]}}, {"referenceToLCIAMethodDataSet": {"shortDescription": [{"value": "Abiotic depletion potential for non fossil resources (ADPE)", "lang": "en"}, {"value": "Potenzial für den abiotischen Abbau nicht fossiler Ressourcen (ADPE)", "lang": "de"}], "type": "LCIA method data set", "refObjectId": "b2ad6494-c78d-11e6-9d9d-cec0c932ce01", "uri": "../lciamethods/b2ad6494-c78d-11e6-9d9d-cec0c932ce01.xml"}, "other": {"anies": [{"name": "referenceToUnitGroupDataSet", "value": {"shortDescription": [{"value": "kg Sb eq", "lang": "en"}], "type": "unit group data set", "refObjectId": "54ccd2d9-a32a-4fc2-923d-f2c8c93e89d4", "uri": "../unitgroups/54ccd2d9-a32a-4fc2-923d-f2c8c93e89d4.xml"}}, {"value": "0.00449903592530704", "module": "A1-A3"}, {"value": "0", "module": "C1"}, {"value": "2.65013565513285E-07", "module": "C2"}, {"value": "0", "module": "C3"}, {"value": "1.68496269109713E-07", "module": "C4"}, {"value": "-0.00315947488342252", "module": "D"}]}}, {"referenceToLCIAMethodDataSet": {"shortDescription": [{"value": "Abiotic depletion potential for fossil resources (ADPF)", "lang": "en"}, {"value": "Potenzial für den abiotischen Abbau fossiler Brennstoffe (ADPF)", "lang": "de"}], "type": "LCIA method data set", "refObjectId": "b2ad6110-c78d-11e6-9d9d-cec0c932ce01", "uri": "../lciamethods/b2ad6110-c78d-11e6-9d9d-cec0c932ce01.xml"}, "other": {"anies": [{"name": "referenceToUnitGroupDataSet", "value": {"shortDescription": [{"value": "MJ", "lang": "en"}], "type": "unit group data set", "refObjectId": "93a60a57-a3c8-11da-a746-0800200c9a66", "uri": "../unitgroups/93a60a57-a3c8-11da-a746-0800200c9a66.xml"}}, {"value": "26764.3893553099", "module": "A1-A3"}, {"value": "0", "module": "C1"}, {"value": "39.8249241581825", "module": "C2"}, {"value": "0", "module": "C3"}, {"value": "35.5528764029718", "module": "C4"}, {"value": "-12638.7757580749", "module": "D"}]}}, {"referenceToLCIAMethodDataSet": {"shortDescription": [{"value": "Water use (WDP)", "lang": "en"}, {"value": "Wassernutzung (WDP)", "lang": "de"}], "type": "LCIA method data set", "refObjectId": "b2ad66ce-c78d-11e6-9d9d-cec0c932ce01", "uri": "../lciamethods/b2ad66ce-c78d-11e6-9d9d-cec0c932ce01.xml"}, "other": {"anies": [{"name": "referenceToUnitGroupDataSet", "value": {"shortDescription": [{"value": "m^(3) world eq deprived", "lang": "en"}], "type": "unit group data set", "refObjectId": "6ae2df01-888e-46c8-b17d-49fa3869b476", "uri": "../unitgroups/6ae2df01-888e-46c8-b17d-49fa3869b476.xml"}}, {"value": "501.296888065899", "module": "A1-A3"}, {"value": "0", "module": "C1"}, {"value": "0.0277457256015725", "module": "C2"}, {"value": "0", "module": "C3"}, {"value": "-0.0289389620167935", "module": "C4"}, {"value": "-284.942824025827", "module": "D"}]}}, {"referenceToLCIAMethodDataSet": {"shortDescription": [{"value": "Incidence of disease due to PM emissions (PM)", "lang": "en"}, {"value": "Auftreten von Krankheiten aufgrund von Feinstaubemissionen (PM)", "lang": "de"}], "type": "LCIA method data set", "refObjectId": "b5c602c6-def3-11e6-bf01-fe55135034f3", "uri": "../lciamethods/b5c602c6-def3-11e6-bf01-fe55135034f3.xml"}, "other": {"anies": [{"name": "referenceToUnitGroupDataSet", "value": {"shortDescription": [{"value": "Disease incidence", "lang": "en"}], "type": "unit group data set", "refObjectId": "3883559b-648f-4afc-8ba2-0bd24f3affa3", "uri": "../unitgroups/3883559b-648f-4afc-8ba2-0bd24f3affa3.xml"}}, {"module": "A1-A3"}, {"module": "C1"}, {"module": "C2"}, {"module": "C3"}, {"module": "C4"}, {"module": "D"}]}}, {"referenceToLCIAMethodDataSet": {"shortDescription": [{"value": "Human exposure efficiency relative to U235 (IR)", "lang": "en"}, {"value": "Wirkung durch Exposition des Menschen mit U235 (IR)", "lang": "de"}], "type": "LCIA method data set", "refObjectId": "b5c632be-def3-11e6-bf01-fe55135034f3", "uri": "../lciamethods/b5c632be-def3-11e6-bf01-fe55135034f3.xml"}, "other": {"anies": [{"name": "referenceToUnitGroupDataSet", "value": {"shortDescription": [{"value": "kBq U235 eq", "lang": "en"}], "type": "unit group data set", "refObjectId": "456b05bf-1415-44a9-9993-02452f554c09", "uri": "../unitgroups/456b05bf-1415-44a9-9993-02452f554c09.xml"}}, {"module": "A1-A3"}, {"module": "C1"}, {"module": "C2"}, {"module": "C3"}, {"module": "C4"}, {"module": "D"}]}}, {"referenceToLCIAMethodDataSet": {"shortDescription": [{"value": "Comparative toxic unit for ecosystems (ETP-fw)", "lang": "en"}, {"value": "Toxizitätsvergleichseinheit für Ökosysteme (ETP-fw)", "lang": "de"}], "type": "LCIA method data set", "refObjectId": "ee1082d1-b0f7-43ca-a1f0-21e2a4a74511", "uri": "../lciamethods/ee1082d1-b0f7-43ca-a1f0-21e2a4a74511.xml"}, "other": {"anies": [{"name": "referenceToUnitGroupDataSet", "value": {"shortDescription": [{"value": "CTUe", "lang": "en"}], "type": "unit group data set", "refObjectId": "aa959ded-f1eb-4efb-9c5c-2d60be36b3e6", "uri": "../unitgroups/aa959ded-f1eb-4efb-9c5c-2d60be36b3e6.xml"}}, {"module": "A1-A3"}, {"module": "C1"}, {"module": "C2"}, {"module": "C3"}, {"module": "C4"}, {"module": "D"}]}}, {"referenceToLCIAMethodDataSet": {"shortDescription": [{"value": "Comparative toxic unit for humans (carcinogenic) (HTP-c)", "lang": "en"}, {"value": "Toxizitätsvergleichseinheit für Menschen (krebserregend) (HTP-c)", "lang": "de"}], "type": "LCIA method data set", "refObjectId": "2299222a-bbd8-474f-9d4f-4dd1f18aea7c", "uri": "../lciamethods/2299222a-bbd8-474f-9d4f-4dd1f18aea7c.xml"}, "other": {"anies": [{"name": "referenceToUnitGroupDataSet", "value": {"shortDescription": [{"value": "CTUh", "lang": "en"}], "type": "unit group data set", "refObjectId": "d4c9523e-2d7e-49fd-8469-998f547d3a70", "uri": "../unitgroups/d4c9523e-2d7e-49fd-8469-998f547d3a70.xml"}}, {"module": "A1-A3"}, {"module": "C1"}, {"module": "C2"}, {"module": "C3"}, {"module": "C4"}, {"module": "D"}]}}, {"referenceToLCIAMethodDataSet": {"shortDescription": [{"value": "Comparative toxic unit for humans (noncarcinogenic) (HTP-nc)", "lang": "en"}, {"value": "Toxizitätsvergleichseinheit für Menschen (nicht krebserregend) (HTP-nc)", "lang": "de"}], "type": "LCIA method data set", "refObjectId": "3af763a5-b7a1-48c9-9cee-1f223481fcef", "uri": "../lciamethods/3af763a5-b7a1-48c9-9cee-1f223481fcef.xml"}, "other": {"anies": [{"name": "referenceToUnitGroupDataSet", "value": {"shortDescription": [{"value": "CTUh", "lang": "en"}], "type": "unit group data set", "refObjectId": "d4c9523e-2d7e-49fd-8469-998f547d3a70", "uri": "../unitgroups/d4c9523e-2d7e-49fd-8469-998f547d3a70.xml"}}, {"module": "A1-A3"}, {"module": "C1"}, {"module": "C2"}, {"module": "C3"}, {"module": "C4"}, {"module": "D"}]}}, {"referenceToLCIAMethodDataSet": {"shortDescription": [{"value": "Soil quality index (SQP)", "lang": "en"}, {"value": "Bodenqualitätsindex (SQP)", "lang": "de"}], "type": "LCIA method data set", "refObjectId": "b2ad6890-c78d-11e6-9d9d-cec0c932ce01", "uri": "../lciamethods/b2ad6890-c78d-11e6-9d9d-cec0c932ce01.xml"}, "other": {"anies": [{"name": "referenceToUnitGroupDataSet", "value": {"shortDescription": [{"value": "SQP", "lang": "en"}], "type": "unit group data set", "refObjectId": "f130951c-e67f-4f7f-8dd4-665de3974e18", "uri": "../unitgroups/f130951c-e67f-4f7f-8dd4-665de3974e18.xml"}}, {"module": "A1-A3"}, {"module": "C1"}, {"module": "C2"}, {"module": "C3"}, {"module": "C4"}, {"module": "D"}]}}]}, "otherAttributes": {"{http://www.indata.network/EPD/2019}epd-version": "1.2"}, "version": "1.1", "locations": "../ILCDLocations.xml"}