{"processInformation": {"dataSetInformation": {"UUID": "4029b66c-591d-4bdf-9842-f34aa74c8f40", "name": {"baseName": [{"value": "Green roof intensive with stainless steel railing", "lang": "en"}, {"value": "Gründach intensiv mit Edelstahlgeländer", "lang": "de"}]}, "classificationInformation": {"classification": [{"class": [{"value": "Komposite", "level": 0, "classId": "10"}, {"value": "Systembauteile", "level": 1, "classId": "10.1"}, {"value": "Dachaufbauten", "level": 2, "classId": "10.1.09"}], "name": "oekobau.dat"}]}, "generalComment": [{"value": "Dieser Datensatz wurde nach dem European Standard EN 15804+A2 für Nachhaltiges Bauen modelliert. Ergebnisse werden in Modulen abgebildet, die den strukturierten Ausdruck von Ergebnissen über den gesamten Lebenszyklus zulassen.", "lang": "de"}], "other": {"anies": [{"margins": 0, "description": [{"lang": "en"}, {"lang": "de"}]}]}}, "quantitativeReference": {"referenceToReferenceFlow": [100019], "type": "Reference flow(s)"}, "time": {"referenceYear": 2023, "dataSetValidUntil": 2026, "timeRepresentativenessDescription": [{"value": "Annual average", "lang": "en"}, {"value": "Jährlicher Durchschnitt", "lang": "de"}]}, "geography": {"locationOfOperationSupplyOrProduction": {"descriptionOfRestrictions": [{"value": "The data set represents the country specific situation in Germany, focusing on the main technologies, the region specific characteristics and / or import statistics.", "lang": "en"}, {"value": "Der Datensatz bildet die länderspezifische Situation in Deutschland ab. Dabei werden Haupttechnologien, spezifische regionale Charakteristiken und ggf. Importstatistiken berücksichtigt.", "lang": "de"}], "location": "DE"}}, "technology": {"technologyDescriptionAndIncludedProcesses": [{"value": "Green roof systems consist of several system components (structure from bottom to top): Root protection foil, protective mat, drainage element, filter fleece, substrate, planting, edge cover and railing. \"Fabrication\" is accomplished by placing the individual components in layers or stages on the building site. The primary roof waterproofing is typically not part of the green roof system.\n\n\n\nDescription of life cycle stages modeled:\n\nModules A1-A3: The balanced green roof system consists of the following materials (in terms of one square meter): root protection film (TPO) 1.2kg, protective mat (PET) 0.5kg, drainage element (PE-HD) 2.2kg, filter fleece (PP) 0.3kg, substrate (including crushed used clay bricks, light volcanic bulk materials, compost, peat) 460kg, planting 25kg, edge cover (galvanized steel sheet) 1.92kg and railing (stainless steel) 3kg.\nThe production of the substrate as well as the metal components dominate the life cycle assessment .\n\n\nModule A4: A truck transport to the building site at a distance of 100 kilometers was considered. The transport distance can be adjusted at the building level if necessary.\n\nModule A5: For the construction, it is assumed that the substrate is transported to the roof with vacuum. Per ton of substrate, 1.5kg of diesel consumption was assumed in an internal combustion engine.\n\nModule C1: For deconstruction, it is assumed that the substrate is transported from the roof with vacuum. Per ton of substrate, 1.5kg of diesel consumption in an internal combustion engine was assumed.\n\nModule C2: For the transport to the rubble processing 50 km (truck, 40 tons EURO6) were assumed.\n\nModule C3: Thermal treatment is accounted for all plastic components.\n\nModule C4: The substrate is sent to landfill. Recycling is theoretically possible, but not common.\nModule D: Metals are assumed to be recycled, with loads for recycling and credits for substitution of primary materials reported in Module D. Module D also includes credits from thermal processing (from Module C3).", "lang": "en"}, {"value": "Gründachsysteme bestehen aus mehreren Systemkomponenten (Aufbau von unten nach oben): Wurzelschutzfolie, Schutzmatte, Drainage Element, Filter Vlies, Substrat, Bepflanzung, Randabdeckung und Geländer. Die \"\"Herstellung\"\" erfolgt durch schicht- bzw. schrittweises Einbringen der einzelnen Komponenten auf der Baustelle. Die primäre Dachabdichtung ist üblicherweise nicht Teil des Gründachsystems.\n\n\n\nBeschreibung der modellierten Lebenszyklusphasen:\n\nModule A1-A3: Das bilanzierte Gründachsystem besteht (in Bezug auf einen Quadratmeter) aus folgenden Materialien: Wurzelschutzfolie (TPO) 1,2kg, Schutzmatte (PET) 0,5kg, Drainage Element (PE-HD) 2,2kg, Filter Vlies (PP) 0,3kg, Substrat (u.a.zerkleinerte gebrauchte Tonziegel, leichte vulkanische Schüttstoffe, Kompost, Torf) 460kg, Bepflanzung 25kg, Randabdeckung (Stahlblech verzinkt) 1,92kg und Geländer (Edelstahl) 3kg.\nDie Herstellung des Substrats sowie der Metallkomponenten dominieren dabei die Ökobilanz .\n\n\nModul A4: Ein LKW-Transport zur Baustelle bei einer Entfernung von 100 Kilometern wurde berücksichtigt. Die Transportentfernung kann auf Gebäudeebene, falls erforderlich, angepasst werden.\n\nModul A5: Für den Aufbau wird davon ausgegangen, dass das Substrat mit Vakuum auf das Dach transportiert wird. Pro t Substrat wurde von 1,5kg Dieselverbrauch in einem Verbrennungsmotor ausgegangen.\n\nModul C1: Für den Rückbau wird davon ausgegangen, dass das Substrat mit Vakuum vom Dach transportiert wird. Pro t Substrat wurde von 1,5kg Dieselverbrauch in einem Verbrennungsmotor ausgegangen.\n\nModul C2: Für den Transport zur Bauschuttaufbereitung wurden 50 km (LKW, 40 Tonnen EURO6) angesetzt.\n\nModul C3: Für alle Kunststoffkomponenten wird eine thermische Verwertung bilanziert.\n\nModul C4: Das Substrat wird einer Deponierung zugeführt. Ein Recycling ist zwar theoretisch möglich, aber nicht gebräuchlich.\n\nModul D: Für Metalle wird ein stoffliches Recycling angenommen, wobei die Lasten für das Recycling und die Gutschriften für die Substitution von Primärmaterial in Modul D ausgewiesen werden. Modul D enthält außerdem Gutschriften aus thermischer Verwertung (aus Modul C3).", "lang": "de"}], "technologicalApplicability": [{"value": "Green roof systems for intensive use are vegetated parts of buildings, with a mix of flat-ball plants, shrubs and small-growing tree species usually used for planting. \nIntensive use means that regular use and maintenance of the area, e.g. as a roof garden, is intended. \nThe high system weight usually results in increased structural requirements for the building. In urban areas, green roof systems improve the microclimate and provide a habitat for a wide variety of organisms. High rainwater retention results in positive effects during heavy rainfall events. In addition, green roof systems contribute to summer and winter thermal insulation as well as sound insulation of underlying building parts.", "lang": "en"}, {"value": "Gründachsysteme für die intensive Benutzung sind begrünte Gebäudeteile, wobei als Bepflanzung üblicherweise ein Mix aus Flachballenpflanzen, Sträuchern und kleinwüchsigen Baumarten eingesetzt wird. \nIntensive Nutzung bedeutet, dass eine regelmäßige Nutzung und Pflege der Fläche, z.B. als Dachgarten, vorgesehen ist. \nDurch die hohe Eigenlast ergeben sich üblicherweise erhöhte Anforderungen an die Statik des Gebäudes. In urbanen Gebieten verbessern Gründachsysteme das Mikroklima und bieten einen Lebensraum für unterschiedlichste Organismen. Durch eine hohe Regenwasserretention ergeben sich positive Effekte bei Starkregenereignissen. Darüber hinaus tragen Gründachsysteme zum sommerlichen und winterlichen Wärmeschutz sowie zum Schallschutz darunterliegender Gebäudeteile bei.", "lang": "de"}]}}, "modellingAndValidation": {"LCIMethodAndAllocation": {"typeOfDataSet": "EPD", "other": {"anies": [{"name": "subType", "value": "generic dataset"}]}}, "dataSourcesTreatmentAndRepresentativeness": {"referenceToDataSource": [{"shortDescription": [{"value": "Documentation of data quality management", "lang": "en"}], "type": "source data set", "refObjectId": "e3bd9bbf-2c3c-42aa-8892-fd13f1065ca5", "version": "24.01.000", "uri": "../sources/e3bd9bbf-2c3c-42aa-8892-fd13f1065ca5.xml"}, {"shortDescription": [{"value": "GaBi Database Edition 2021, CUP2021.01", "lang": "en"}], "type": "source data set", "refObjectId": "1cece811-7501-44d4-8067-9259bd5cb835", "version": "00.01.000", "uri": "../sources/1cece811-7501-44d4-8067-9259bd5cb835.xml"}, {"shortDescription": [{"value": "Sphera Managed LCA Content Databases (all versions)", "lang": "en"}], "type": "source data set", "refObjectId": "28d74cc0-db8b-4d7e-bc44-5f6d56ce0c4a", "version": "00.03.002", "uri": "../sources/28d74cc0-db8b-4d7e-bc44-5f6d56ce0c4a.xml"}], "useAdviceForDataSet": [{"value": "This data record refers to the production of 1m² green roof system (intensive use) including stainless steel railings and planting. The weight per piece area is approx. 494 kg/m² (dry) with a structure height of approx. 50cm (of which 45 cm are lower and upper substrate). The data set can be approximately linearly scaled (by mass) for estimating other weights per unit area between 400 and 600 kg/m². However, the system composition (see field \"technical description of the product system over the life cycle\") must be taken into account.\n\n\n\nFor the modeling, information from a manufacturing company (primary data) was used both in terms of material composition and for manufacturing efforts. \n\n\n\nEstimates and assumptions:\n\nUsed brick material used in the substrate enters the system as load free secondary material. An electricity consumption of 0.05 MJ/kg is estimated for the crushing of bricks to brick rubble. \n\n\n\nCompost from green waste is treated load-free (with respect to its production), since it is assumed that the green waste reaches the end of waste status only after the composting process. Furthermore, it is assumed that the biog. C-content in the compost is 13.9 M.%. This carbon is balanced as CO2 uptake in module A1, namely 0.51 kg CO2/kg compost. The sequestered carbon dioxide is released again in module C4 (landfill) (carbon neutrality\"\").       \nAll plastics are modeled as primary plastics, although recycled materials are often used in practice (conservative approach).\n\n\n\nA comparatively small roof size of 10 x 10 m was assumed for sheet metal covers (galvanized steel sheet) and penetration-free stainless steel railing (conservative approach). Per square meter, 1.92 kg of galvanized sheet steel and 3 kg of stainless steel were taken into account. In practice, and especially for larger roof areas, significantly lower quantities per square meter are possible here.\n\n\n\nSmaller system components (e.g. drain boxes) were neglected (cut-off criteria).\n\n\n\nOverall, a very good representativeness can be assumed under ecobalance-conservative boundary conditions.", "lang": "en"}, {"value": "Dieser Datensatz bezieht sich auf die Herstellung von 1m² Gründachsystem (intensive Nutzung) inklusive Geländer aus Edelstahl und Bepflanzung. Das Flächengewicht beträgt ca. 494 kg/m² (trocken) bei einer Aufbauhöhe von ca. 50cm (davon 45 cm Unter- und Obersubstrat). Der Datensatz kann für die Abschätzung anderer Flächengewichte zwischen 400 und 600 kg/m² näherungsweise linear (über die Masse) skaliert werden. Hierbei ist jedoch die Systemzusammensetzung (siehe Feld \"technische Beschreibung des Produktsystems über den Lebenszyklus\") zu beachten.\n\n\n\nFür die Modellierung wurden Informationen einer Herstellfirma (Primärdaten) sowohl in Bezug auf die stoffliche Zusammensetzung als auch für die Herstellungsaufwendungen zugrunde gelegt. \n\n\n\nAbschätzungen und Annahmen:\n\nGebrauchtes Ziegelmaterial, welches im Substrat verwendet wird, geht lastenfrei in das System ein. Für die Zerkleinerung von Ziegeln zu Ziegelbruch wird ein Stromverbrauch von 0,05 MJ/kg abgeschätzt. \n\nKompost aus Grünschnitt wird (in Bezug auf dessen Herstellung) lastenfrei behandelt, da angenommen wird, dass der Grünschnitt das Ende der Abfalleigenschaft erst nach der Kompostierung erreicht. Weiterhin wird von einem biog. C-Gehalt im Kompost von 13,9 M.% ausgegangen . Dieser Kohlenstoff wird als CO2-Aufnahme in Modul A1 bilanziert, und zwar 0,51 kg CO2/kg Kompost. Das gebundene Kohlenstoffdioxid wird in Modul C4 (Deponierung) wieder freigesetzt (\"carbon neutrality\").\n\n \n\nAlle Kunststoffe werden als Primärkunststoffe modelliert, wenngleich in der Praxis häufig Recyclingmaterialien eingesetzt werden (konservativer Ansatz).\n\n\n\nFür Blechabdeckungen (Stahlblech verzinkt) und durchdringungsfreies Edelstahlgeländer wurde von einer vergleichsweise kleinen Dachgröße von 10 x 10 m ausgegangen (konservativer Ansatz). Pro Quadratmeter wurden 1,92 kg Stahlblech verzinkt und 3 kg Edelstahl berücksichtigt. In der Praxis und insbesondere bei größeren Dachflächen, sind hier deutlich niedrigere Mengen pro Quadratmeter möglich.\n\n\n\nKleinere Systemkomponenten (z.B. Ablaufkästen) wurden vernachlässigt (Abschneidekriterium).\n\n\n\nInsgesamt kann von einer sehr guten Repräsentativität unter ökobilanziell konservativen Randbedingungen ausgegangen werden.", "lang": "de"}]}, "validation": {"review": [{"referenceToNameOfReviewerAndInstitution": [{"shortDescription": [{"value": "Sphera Solutions GmbH", "lang": "en"}], "type": "contact data set", "refObjectId": "d7fa0337-f279-430d-becf-7f3111a85010", "version": "24.01.000", "uri": "../contacts/d7fa0337-f279-430d-becf-7f3111a85010.xml"}], "type": "Dependent internal review"}, {"referenceToNameOfReviewerAndInstitution": [{"shortDescription": [{"value": "Sphera Product Sustainability user forum", "lang": "en"}], "type": "contact data set", "refObjectId": "8f1306f0-7b83-4f36-a537-aa83f0498266", "version": "24.01.000", "uri": "../contacts/8f1306f0-7b83-4f36-a537-aa83f0498266.xml"}], "type": "Independent external review"}]}, "complianceDeclarations": {"compliance": [{"referenceToComplianceSystem": {"shortDescription": [{"value": "EN 15804+A2 (EF 3.1)", "lang": "de"}, {"value": "EN 15804+A2 (EF 3.1)", "lang": "en"}], "type": "source data set", "refObjectId": "d4aa3ec7-b1d7-4a4a-a6cb-37af88dcc902", "version": "00.01.000", "uri": "../sources/d4aa3ec7-b1d7-4a4a-a6cb-37af88dcc902.xml"}, "approvalOfOverallCompliance": "Fully compliant"}]}}, "administrativeInformation": {"dataGenerator": {"referenceToPersonOrEntityGeneratingTheDataSet": [{"shortDescription": [{"value": "Sphera Solutions GmbH", "lang": "en"}], "type": "contact data set", "refObjectId": "d7fa0337-f279-430d-becf-7f3111a85010", "version": "24.01.000", "uri": "../contacts/d7fa0337-f279-430d-becf-7f3111a85010.xml"}]}, "dataEntryBy": {"timeStamp": 1718121637000, "referenceToDataSetFormat": [{"shortDescription": [{"value": "ILCD format 1.1", "lang": "de"}, {"value": "ILCD format 1.1", "lang": "en"}], "type": "source data set", "refObjectId": "a97a0155-0234-4b87-b4ce-a45da52f2a40", "version": "01.00.000", "uri": "../sources/a97a0155-0234-4b87-b4ce-a45da52f2a40.xml"}, {"shortDescription": [{"value": "EPD-Datenformaterweiterungen v1.2", "lang": "de"}, {"value": "EPD Data Format Extensions v1.2", "lang": "en"}], "type": "source data set", "refObjectId": "a29449fd-aa2f-4de8-b5d7-4b06b43c6fde", "version": "00.01.000", "uri": "../sources/a29449fd-aa2f-4de8-b5d7-4b06b43c6fde.xml"}], "referenceToPersonOrEntityEnteringTheData": {"shortDescription": [{"value": "Sphera Solutions GmbH", "lang": "en"}], "type": "contact data set", "refObjectId": "d7fa0337-f279-430d-becf-7f3111a85010", "version": "24.01.000", "uri": "../contacts/d7fa0337-f279-430d-becf-7f3111a85010.xml"}}, "publicationAndOwnership": {"dataSetVersion": "20.24.070", "referenceToPrecedingDataSetVersion": [{"shortDescription": [{"value": "Green roof intensive with stainless steel railing", "lang": "en"}], "type": "process data set", "refObjectId": "a1f68d1e-35b8-4a44-8200-e030a7b23135", "uri": "https://www.oekobaudat.de/OEKOBAU.DAT/resource/processes/a1f68d1e-35b8-4a44-8200-e030a7b23135?version=20.23.050"}], "referenceToRegistrationAuthority": {"shortDescription": [{"value": "Sphera Solutions GmbH", "lang": "en"}], "type": "contact data set", "refObjectId": "d7fa0337-f279-430d-becf-7f3111a85010", "version": "24.01.000", "uri": "../contacts/d7fa0337-f279-430d-becf-7f3111a85010.xml"}, "referenceToOwnershipOfDataSet": {"shortDescription": [{"value": "Sphera Solutions GmbH", "lang": "en"}], "type": "contact data set", "refObjectId": "d7fa0337-f279-430d-becf-7f3111a85010", "version": "24.01.000", "uri": "../contacts/d7fa0337-f279-430d-becf-7f3111a85010.xml"}, "copyright": true, "licenseType": "Free of charge for all users and uses", "accessRestrictions": [{"value": "The license conditions as stated on https://www.oekobaudat.de/apply.", "lang": "en"}, {"value": "Es gelten die Lizenzbedingungen wie sie auf https://www.oekobaudat.de/ genannt sind.", "lang": "de"}], "other": {"anies": [{"name": "referenceToPublisher", "value": {"shortDescription": [{"value": "BBSR", "lang": "en"}], "type": "contact data set", "refObjectId": "f11651e0-7877-11e3-981f-0800200c9a66", "version": "00.01.000", "uri": "../contacts/f11651e0-7877-11e3-981f-0800200c9a66.xml"}}]}}}, "exchanges": {"exchange": [{"dataSetInternalID": 100019, "referenceToFlowDataSet": {"shortDescription": [{"value": "Green roof intensive with stainless steel railing", "lang": "en"}, {"value": "Gründach intensiv mit Edelstahlgeländer", "lang": "de"}], "type": "flow data set", "refObjectId": "2677859d-4cbe-4f89-995d-24d54debe4f1", "version": "24.01.000", "uri": "../flows/2677859d-4cbe-4f89-995d-24d54debe4f1.xml"}, "meanAmount": 1.0, "referenceFlow": true, "resultingflowAmount": 1.0, "flowProperties": [{"name": [{"lang": "en", "value": "Area"}, {"lang": "de", "value": "Fläche"}], "uuid": "93a60a56-a3c8-19da-a746-0800200c9a66", "referenceFlowProperty": true, "meanValue": 1.0, "referenceUnit": "qm", "unitGroupUUID": "c20a03d7-bd90-4569-bc94-66cfd364dfc8"}], "materialProperties": [{"name": "grammage", "value": "494.0", "unit": "kg/m^2", "unitDescription": "kilograms per square meter"}], "typeOfFlow": "Product flow", "classification": {"classHierarchy": "Valuable substances / Materials / Minerals", "name": "GaBiCategories"}}, {"dataSetInternalID": 100020, "referenceToFlowDataSet": {"shortDescription": [{"value": "Use of renewable primary energy as energy carrier (PERE)", "lang": "en"}, {"value": "Erneuerbare Primärenergie als Energieträger (PERE)", "lang": "de"}], "type": "flow data set", "refObjectId": "20f32be5-0398-4288-9b6d-accddd195317", "version": "24.01.000", "uri": "../flows/20f32be5-0398-4288-9b6d-accddd195317.xml"}, "exchange direction": "INPUT", "other": {"anies": [{"value": "97.6087885842135", "module": "A1-A3"}, {"name": "referenceToUnitGroupDataSet", "value": {"shortDescription": [{"value": "MJ", "lang": "en"}], "type": "unit group data set", "refObjectId": "93a60a57-a3c8-11da-a746-0800200c9a66", "version": "03.00.000", "uri": "../unitgroups/93a60a57-a3c8-11da-a746-0800200c9a66.xml"}}, {"value": "4.03748732140098", "module": "A4"}, {"value": "0.000731909684592242", "module": "C1"}, {"value": "2.56307038415927", "module": "C2"}, {"value": "0.688952059989664", "module": "C3"}, {"value": "-956.432264411279", "module": "C4"}, {"value": "-45.4924314872973", "module": "D"}]}, "resolvedFlowVersion": "38.00.000", "flowProperties": [], "typeOfFlow": "Other flow", "classification": {"classHierarchy": "Quantities", "name": "GaBiCategories"}}, {"dataSetInternalID": 100021, "referenceToFlowDataSet": {"shortDescription": [{"value": "Use of renewable primary energy resources used as raw materials (PERM)", "lang": "en"}, {"value": "Erneuerbare Primärenergie zur stofflichen Nutzung (PERM)", "lang": "de"}], "type": "flow data set", "refObjectId": "fb3ec0de-548d-4508-aea5-00b73bf6f702", "version": "24.01.000", "uri": "../flows/fb3ec0de-548d-4508-aea5-00b73bf6f702.xml"}, "exchange direction": "INPUT", "other": {"anies": [{"value": "979.7", "module": "A1-A3"}, {"name": "referenceToUnitGroupDataSet", "value": {"shortDescription": [{"value": "MJ", "lang": "en"}], "type": "unit group data set", "refObjectId": "93a60a57-a3c8-11da-a746-0800200c9a66", "version": "03.00.000", "uri": "../unitgroups/93a60a57-a3c8-11da-a746-0800200c9a66.xml"}}, {"value": "0", "module": "A4"}, {"value": "0", "module": "C1"}, {"value": "0", "module": "C2"}, {"value": "0", "module": "C3"}, {"value": "0", "module": "C4"}, {"value": "0", "module": "D"}]}, "resolvedFlowVersion": "38.00.000", "flowProperties": [], "typeOfFlow": "Other flow", "classification": {"classHierarchy": "Quantities", "name": "GaBiCategories"}}, {"dataSetInternalID": 100022, "referenceToFlowDataSet": {"shortDescription": [{"value": "Total use of renewable primary energy (PERT)", "lang": "en"}, {"value": "Total erneuerbare Primärenergie (PERT)", "lang": "de"}], "type": "flow data set", "refObjectId": "53f97275-fa8a-4cdd-9024-65936002acd0", "version": "24.01.000", "uri": "../flows/53f97275-fa8a-4cdd-9024-65936002acd0.xml"}, "exchange direction": "INPUT", "other": {"anies": [{"value": "1077.30878858421", "module": "A1-A3"}, {"name": "referenceToUnitGroupDataSet", "value": {"shortDescription": [{"value": "MJ", "lang": "en"}], "type": "unit group data set", "refObjectId": "93a60a57-a3c8-11da-a746-0800200c9a66", "version": "03.00.000", "uri": "../unitgroups/93a60a57-a3c8-11da-a746-0800200c9a66.xml"}}, {"value": "4.03748732140098", "module": "A4"}, {"value": "0.000731909684592242", "module": "C1"}, {"value": "2.56307038415927", "module": "C2"}, {"value": "0.688952059989664", "module": "C3"}, {"value": "-956.432264411279", "module": "C4"}, {"value": "-45.4924314872973", "module": "D"}]}, "resolvedFlowVersion": "38.00.000", "flowProperties": [], "typeOfFlow": "Other flow", "classification": {"classHierarchy": "Quantities / Environmental quantities / EPD EN 15804 / LCI indicators", "name": "GaBiCategories"}}, {"dataSetInternalID": 100023, "referenceToFlowDataSet": {"shortDescription": [{"value": "Use of non renewable primary energy as energy carrier (PENRE)", "lang": "en"}, {"value": "Nicht-erneuerbare Primärenergie als Energieträger (PENRE)", "lang": "de"}], "type": "flow data set", "refObjectId": "ac857178-2b45-46ec-892a-a9a4332f0372", "version": "24.01.000", "uri": "../flows/ac857178-2b45-46ec-892a-a9a4332f0372.xml"}, "exchange direction": "INPUT", "other": {"anies": [{"value": "987.511901522925", "module": "A1-A3"}, {"name": "referenceToUnitGroupDataSet", "value": {"shortDescription": [{"value": "MJ", "lang": "en"}], "type": "unit group data set", "refObjectId": "93a60a57-a3c8-11da-a746-0800200c9a66", "version": "03.00.000", "uri": "../unitgroups/93a60a57-a3c8-11da-a746-0800200c9a66.xml"}}, {"value": "47.7579338441609", "module": "A4"}, {"value": "0.00674404471137149", "module": "C1"}, {"value": "23.160101913454", "module": "C2"}, {"value": "179.823772600219", "module": "C3"}, {"value": "177.796659437772", "module": "C4"}, {"value": "-169.747619308271", "module": "D"}]}, "resolvedFlowVersion": "38.00.000", "flowProperties": [], "typeOfFlow": "Other flow", "classification": {"classHierarchy": "Quantities", "name": "GaBiCategories"}}, {"dataSetInternalID": 100024, "referenceToFlowDataSet": {"shortDescription": [{"value": "Use of non renewable primary energy resources used as raw materials (PENRM)", "lang": "en"}, {"value": "Nicht-erneuerbare Primärenergie zur stofflichen Nutzung (PENRM)", "lang": "de"}], "type": "flow data set", "refObjectId": "1421caa0-679d-4bf4-b282-0eb850ccae27", "version": "24.01.000", "uri": "../flows/1421caa0-679d-4bf4-b282-0eb850ccae27.xml"}, "exchange direction": "INPUT", "other": {"anies": [{"value": "177.85", "module": "A1-A3"}, {"name": "referenceToUnitGroupDataSet", "value": {"shortDescription": [{"value": "MJ", "lang": "en"}], "type": "unit group data set", "refObjectId": "93a60a57-a3c8-11da-a746-0800200c9a66", "version": "03.00.000", "uri": "../unitgroups/93a60a57-a3c8-11da-a746-0800200c9a66.xml"}}, {"value": "0", "module": "A4"}, {"value": "0", "module": "C1"}, {"value": "0", "module": "C2"}, {"value": "-177.85", "module": "C3"}, {"value": "0", "module": "C4"}, {"value": "0", "module": "D"}]}, "resolvedFlowVersion": "38.00.000", "flowProperties": [], "typeOfFlow": "Other flow", "classification": {"classHierarchy": "Quantities", "name": "GaBiCategories"}}, {"dataSetInternalID": 100025, "referenceToFlowDataSet": {"shortDescription": [{"value": "Total use of non renewable primary energy resource (PENRT)", "lang": "en"}, {"value": "Total nicht-erneuerbare Primärenergie (PENRT)", "lang": "de"}], "type": "flow data set", "refObjectId": "06159210-646b-4c8d-8583-da9b3b95a6c1", "version": "24.01.000", "uri": "../flows/06159210-646b-4c8d-8583-da9b3b95a6c1.xml"}, "exchange direction": "INPUT", "other": {"anies": [{"value": "1165.36190152292", "module": "A1-A3"}, {"name": "referenceToUnitGroupDataSet", "value": {"shortDescription": [{"value": "MJ", "lang": "en"}], "type": "unit group data set", "refObjectId": "93a60a57-a3c8-11da-a746-0800200c9a66", "version": "03.00.000", "uri": "../unitgroups/93a60a57-a3c8-11da-a746-0800200c9a66.xml"}}, {"value": "47.7579338441609", "module": "A4"}, {"value": "0.00674404471137149", "module": "C1"}, {"value": "23.160101913454", "module": "C2"}, {"value": "1.97377260021935", "module": "C3"}, {"value": "177.796659437772", "module": "C4"}, {"value": "-169.747619308271", "module": "D"}]}, "resolvedFlowVersion": "38.00.000", "flowProperties": [], "typeOfFlow": "Other flow", "classification": {"classHierarchy": "Quantities / Environmental quantities / EPD EN 15804 / LCI indicators", "name": "GaBiCategories"}}, {"dataSetInternalID": 100026, "referenceToFlowDataSet": {"shortDescription": [{"value": "Use of secondary material (SM)", "lang": "en"}, {"value": "Einsatz von Sekundärstoffen (SM)", "lang": "de"}], "type": "flow data set", "refObjectId": "c6a1f35f-2d09-4f54-8dfb-97e502e1ce92", "version": "24.01.000", "uri": "../flows/c6a1f35f-2d09-4f54-8dfb-97e502e1ce92.xml"}, "exchange direction": "INPUT", "other": {"anies": [{"value": "330.75", "module": "A1-A3"}, {"name": "referenceToUnitGroupDataSet", "value": {"shortDescription": [{"value": "kg", "lang": "en"}], "type": "unit group data set", "refObjectId": "93a60a57-a4c8-11da-a746-0800200c9a66", "version": "03.00.000", "uri": "../unitgroups/93a60a57-a4c8-11da-a746-0800200c9a66.xml"}}, {"value": "0", "module": "A4"}, {"value": "0", "module": "C1"}, {"value": "0", "module": "C2"}, {"value": "0", "module": "C3"}, {"value": "0", "module": "C4"}, {"value": "0", "module": "D"}]}, "resolvedFlowVersion": "38.00.000", "flowProperties": [], "typeOfFlow": "Other flow", "classification": {"classHierarchy": "Quantities / Environmental quantities / EPD EN 15804 / LCI indicators", "name": "GaBiCategories"}}, {"dataSetInternalID": 100027, "referenceToFlowDataSet": {"shortDescription": [{"value": "Use of renewable secondary fuels (SF)", "lang": "en"}, {"value": "Erneuerbare Sekundärbrennstoffe (SF)", "lang": "de"}], "type": "flow data set", "refObjectId": "64333088-a55f-4aa2-9a31-c10b07816787", "version": "24.01.000", "uri": "../flows/64333088-a55f-4aa2-9a31-c10b07816787.xml"}, "exchange direction": "INPUT", "other": {"anies": [{"value": "0", "module": "A1-A3"}, {"name": "referenceToUnitGroupDataSet", "value": {"shortDescription": [{"value": "MJ", "lang": "en"}], "type": "unit group data set", "refObjectId": "93a60a57-a3c8-11da-a746-0800200c9a66", "version": "03.00.000", "uri": "../unitgroups/93a60a57-a3c8-11da-a746-0800200c9a66.xml"}}, {"value": "0", "module": "A4"}, {"value": "0", "module": "C1"}, {"value": "0", "module": "C2"}, {"value": "0", "module": "C3"}, {"value": "0", "module": "C4"}, {"value": "0", "module": "D"}]}, "resolvedFlowVersion": "38.00.000", "flowProperties": [], "typeOfFlow": "Other flow", "classification": {"classHierarchy": "Quantities / Environmental quantities / EPD EN 15804 / LCI indicators", "name": "GaBiCategories"}}, {"dataSetInternalID": 100028, "referenceToFlowDataSet": {"shortDescription": [{"value": "Use of non renewable secondary fuels (NRSF)", "lang": "en"}, {"value": "Nicht erneuerbare Sekundärbrennstoffe (NRSF)", "lang": "de"}], "type": "flow data set", "refObjectId": "89def144-d39a-4287-b86f-efde453ddcb2", "version": "24.01.000", "uri": "../flows/89def144-d39a-4287-b86f-efde453ddcb2.xml"}, "exchange direction": "INPUT", "other": {"anies": [{"value": "0", "module": "A1-A3"}, {"name": "referenceToUnitGroupDataSet", "value": {"shortDescription": [{"value": "MJ", "lang": "en"}], "type": "unit group data set", "refObjectId": "93a60a57-a3c8-11da-a746-0800200c9a66", "version": "03.00.000", "uri": "../unitgroups/93a60a57-a3c8-11da-a746-0800200c9a66.xml"}}, {"value": "0", "module": "A4"}, {"value": "0", "module": "C1"}, {"value": "0", "module": "C2"}, {"value": "0", "module": "C3"}, {"value": "0", "module": "C4"}, {"value": "0", "module": "D"}]}, "resolvedFlowVersion": "38.00.000", "flowProperties": [], "typeOfFlow": "Other flow", "classification": {"classHierarchy": "Quantities / Environmental quantities / EPD EN 15804 / LCI indicators", "name": "GaBiCategories"}}, {"dataSetInternalID": 100029, "referenceToFlowDataSet": {"shortDescription": [{"value": "Net use of fresh water (FW)", "lang": "en"}, {"value": "Nettoeinsatz von Süßwasserressourcen (FW)", "lang": "de"}], "type": "flow data set", "refObjectId": "3cf952c8-f3a4-461d-8c96-96456ca62246", "version": "24.01.000", "uri": "../flows/3cf952c8-f3a4-461d-8c96-96456ca62246.xml"}, "exchange direction": "INPUT", "other": {"anies": [{"value": "0.243284365770978", "module": "A1-A3"}, {"name": "referenceToUnitGroupDataSet", "value": {"shortDescription": [{"value": "m3", "lang": "en"}], "type": "unit group data set", "refObjectId": "93a60a57-a3c8-12da-a746-0800200c9a66", "version": "03.00.000", "uri": "../unitgroups/93a60a57-a3c8-12da-a746-0800200c9a66.xml"}}, {"value": "0.00453406672155413", "module": "A4"}, {"value": "6.9590213861695E-7", "module": "C1"}, {"value": "0.0023944614885794", "module": "C2"}, {"value": "0.0273081234395714", "module": "C3"}, {"value": "0.0291536713489981", "module": "C4"}, {"value": "-0.0625566482442835", "module": "D"}]}, "resolvedFlowVersion": "38.00.000", "flowProperties": [], "typeOfFlow": "Other flow", "classification": {"classHierarchy": "Quantities / Environmental quantities / EPD EN 15804 / LCI indicators", "name": "GaBiCategories"}}, {"dataSetInternalID": 100030, "referenceToFlowDataSet": {"shortDescription": [{"value": "Hazardous waste disposed (HWD)", "lang": "en"}, {"value": "Gefährlicher Abfall zur Deponie (HWD)", "lang": "de"}], "type": "flow data set", "refObjectId": "430f9e0f-59b2-46a0-8e0d-55e0e84948fc", "version": "24.01.000", "uri": "../flows/430f9e0f-59b2-46a0-8e0d-55e0e84948fc.xml"}, "exchange direction": "OUTPUT", "other": {"anies": [{"value": "9.60489932088481E-7", "module": "A1-A3"}, {"name": "referenceToUnitGroupDataSet", "value": {"shortDescription": [{"value": "kg", "lang": "en"}], "type": "unit group data set", "refObjectId": "93a60a57-a4c8-11da-a746-0800200c9a66", "version": "03.00.000", "uri": "../unitgroups/93a60a57-a4c8-11da-a746-0800200c9a66.xml"}}, {"value": "1.54508141039988E-9", "module": "A4"}, {"value": "2.87244302696773E-13", "module": "C1"}, {"value": "1.12752879304379E-9", "module": "C2"}, {"value": "1.57889524655809E-9", "module": "C3"}, {"value": "3.64557755414129E-8", "module": "C4"}, {"value": "-7.9303780140389E-8", "module": "D"}]}, "resolvedFlowVersion": "38.00.000", "flowProperties": [], "typeOfFlow": "Other flow", "classification": {"classHierarchy": "Quantities / Environmental quantities / EPD EN 15804 / LCI indicators", "name": "GaBiCategories"}}, {"dataSetInternalID": 100031, "referenceToFlowDataSet": {"shortDescription": [{"value": "Non harzardous waste disposed (NHWD)", "lang": "en"}, {"value": "Entsorgter nicht gefährlicher Abfall (NHWD)", "lang": "de"}], "type": "flow data set", "refObjectId": "b29ef66b-e286-4afa-949f-62f1a7b4d7fa", "version": "24.01.000", "uri": "../flows/b29ef66b-e286-4afa-949f-62f1a7b4d7fa.xml"}, "exchange direction": "OUTPUT", "other": {"anies": [{"value": "1.72714674852229", "module": "A1-A3"}, {"name": "referenceToUnitGroupDataSet", "value": {"shortDescription": [{"value": "kg", "lang": "en"}], "type": "unit group data set", "refObjectId": "93a60a57-a4c8-11da-a746-0800200c9a66", "version": "03.00.000", "uri": "../unitgroups/93a60a57-a4c8-11da-a746-0800200c9a66.xml"}}, {"value": "0.00742780352789499", "module": "A4"}, {"value": "1.11671919420793E-6", "module": "C1"}, {"value": "0.00391585098608646", "module": "C2"}, {"value": "0.0780675024859032", "module": "C3"}, {"value": "443.389406011373", "module": "C4"}, {"value": "-0.443690757240604", "module": "D"}]}, "resolvedFlowVersion": "38.00.000", "flowProperties": [], "typeOfFlow": "Other flow", "classification": {"classHierarchy": "Quantities / Environmental quantities / EPD EN 15804 / LCI indicators", "name": "GaBiCategories"}}, {"dataSetInternalID": 100032, "referenceToFlowDataSet": {"shortDescription": [{"value": "Radioactive waste disposed (RWD)", "lang": "en"}, {"value": "Entsorgter radioaktiver Abfall (RWD)", "lang": "de"}], "type": "flow data set", "refObjectId": "3449546e-52ad-4b39-b809-9fb77cea8ff6", "version": "24.01.000", "uri": "../flows/3449546e-52ad-4b39-b809-9fb77cea8ff6.xml"}, "exchange direction": "OUTPUT", "other": {"anies": [{"value": "0.00635724734798841", "module": "A1-A3"}, {"name": "referenceToUnitGroupDataSet", "value": {"shortDescription": [{"value": "kg", "lang": "en"}], "type": "unit group data set", "refObjectId": "93a60a57-a4c8-11da-a746-0800200c9a66", "version": "03.00.000", "uri": "../unitgroups/93a60a57-a4c8-11da-a746-0800200c9a66.xml"}}, {"value": "6.17264377757136E-5", "module": "A4"}, {"value": "9.10526515604323E-9", "module": "C1"}, {"value": "3.68631992635882E-5", "module": "C2"}, {"value": "5.86731989373543E-5", "module": "C3"}, {"value": "0.00204492869110154", "module": "C4"}, {"value": "-0.00193252103530615", "module": "D"}]}, "resolvedFlowVersion": "38.00.000", "flowProperties": [], "typeOfFlow": "Other flow", "classification": {"classHierarchy": "Quantities / Environmental quantities / EPD EN 15804 / LCI indicators", "name": "GaBiCategories"}}, {"dataSetInternalID": 100033, "referenceToFlowDataSet": {"shortDescription": [{"value": "Components for re-use (CRU)", "lang": "en"}, {"value": "Komponenten für die Wiederverwendung (CRU)", "lang": "de"}], "type": "flow data set", "refObjectId": "a2b32f97-3fc7-4af2-b209-525bc6426f33", "version": "24.01.000", "uri": "../flows/a2b32f97-3fc7-4af2-b209-525bc6426f33.xml"}, "exchange direction": "OUTPUT", "other": {"anies": [{"value": "0", "module": "A1-A3"}, {"name": "referenceToUnitGroupDataSet", "value": {"shortDescription": [{"value": "kg", "lang": "en"}], "type": "unit group data set", "refObjectId": "93a60a57-a4c8-11da-a746-0800200c9a66", "version": "03.00.000", "uri": "../unitgroups/93a60a57-a4c8-11da-a746-0800200c9a66.xml"}}, {"value": "0", "module": "A4"}, {"value": "0", "module": "C1"}, {"value": "0", "module": "C2"}, {"value": "0", "module": "C3"}, {"value": "0", "module": "C4"}, {"value": "0", "module": "D"}]}, "resolvedFlowVersion": "38.00.000", "flowProperties": [], "typeOfFlow": "Other flow", "classification": {"classHierarchy": "Quantities / Environmental quantities / EPD EN 15804 / LCI indicators", "name": "GaBiCategories"}}, {"dataSetInternalID": 100034, "referenceToFlowDataSet": {"shortDescription": [{"value": "Materials for recycling  (MFR)", "lang": "en"}, {"value": "Stoffe zum Recycling (MFR)", "lang": "de"}], "type": "flow data set", "refObjectId": "d7fe48a5-4103-49c8-9aae-b0b5dfdbd6ae", "version": "24.01.000", "uri": "../flows/d7fe48a5-4103-49c8-9aae-b0b5dfdbd6ae.xml"}, "exchange direction": "OUTPUT", "other": {"anies": [{"value": "0", "module": "A1-A3"}, {"name": "referenceToUnitGroupDataSet", "value": {"shortDescription": [{"value": "kg", "lang": "en"}], "type": "unit group data set", "refObjectId": "93a60a57-a4c8-11da-a746-0800200c9a66", "version": "03.00.000", "uri": "../unitgroups/93a60a57-a4c8-11da-a746-0800200c9a66.xml"}}, {"value": "0", "module": "A4"}, {"value": "3", "module": "C1"}, {"value": "0", "module": "C2"}, {"value": "1.92", "module": "C3"}, {"value": "0", "module": "C4"}, {"value": "0", "module": "D"}]}, "resolvedFlowVersion": "38.00.000", "flowProperties": [], "typeOfFlow": "Other flow", "classification": {"classHierarchy": "Quantities / Environmental quantities / EPD EN 15804 / LCI indicators", "name": "GaBiCategories"}}, {"dataSetInternalID": 100035, "referenceToFlowDataSet": {"shortDescription": [{"value": "Materials for energy recovery (MER)", "lang": "en"}, {"value": "Stoffe für die Energierückgewinnung (MER)", "lang": "de"}], "type": "flow data set", "refObjectId": "59a9181c-3aaf-46ee-8b13-2b3723b6e447", "version": "24.01.000", "uri": "../flows/59a9181c-3aaf-46ee-8b13-2b3723b6e447.xml"}, "exchange direction": "OUTPUT", "other": {"anies": [{"value": "0", "module": "A1-A3"}, {"name": "referenceToUnitGroupDataSet", "value": {"shortDescription": [{"value": "kg", "lang": "en"}], "type": "unit group data set", "refObjectId": "93a60a57-a4c8-11da-a746-0800200c9a66", "version": "03.00.000", "uri": "../unitgroups/93a60a57-a4c8-11da-a746-0800200c9a66.xml"}}, {"value": "0", "module": "A4"}, {"value": "0", "module": "C1"}, {"value": "0", "module": "C2"}, {"value": "0", "module": "C3"}, {"value": "0", "module": "C4"}, {"value": "0", "module": "D"}]}, "resolvedFlowVersion": "38.00.000", "flowProperties": [], "typeOfFlow": "Other flow", "classification": {"classHierarchy": "Quantities / Environmental quantities / EPD EN 15804 / LCI indicators", "name": "GaBiCategories"}}, {"dataSetInternalID": 100036, "referenceToFlowDataSet": {"shortDescription": [{"value": "Exported electrical energy (EEE)", "lang": "en"}, {"value": "Exportierte elektrische Energie (EEE)", "lang": "de"}], "type": "flow data set", "refObjectId": "4da0c987-2b76-40d6-9e9e-82a017aaaf29", "version": "24.01.000", "uri": "../flows/4da0c987-2b76-40d6-9e9e-82a017aaaf29.xml"}, "exchange direction": "OUTPUT", "other": {"anies": [{"value": "0", "module": "A1-A3"}, {"name": "referenceToUnitGroupDataSet", "value": {"shortDescription": [{"value": "MJ", "lang": "en"}], "type": "unit group data set", "refObjectId": "93a60a57-a3c8-11da-a746-0800200c9a66", "version": "03.00.000", "uri": "../unitgroups/93a60a57-a3c8-11da-a746-0800200c9a66.xml"}}, {"value": "0", "module": "A4"}, {"value": "0", "module": "C1"}, {"value": "0", "module": "C2"}, {"value": "22.4949325824344", "module": "C3"}, {"value": "0", "module": "C4"}, {"value": "0", "module": "D"}]}, "resolvedFlowVersion": "38.00.000", "flowProperties": [], "typeOfFlow": "Other flow", "classification": {"classHierarchy": "Quantities / Environmental quantities / EPD EN 15804 / LCI indicators", "name": "GaBiCategories"}}, {"dataSetInternalID": 100037, "referenceToFlowDataSet": {"shortDescription": [{"value": "Exported thermal energy (EET)", "lang": "en"}, {"value": "Exportierte thermische Energie (EET)", "lang": "de"}], "type": "flow data set", "refObjectId": "98daf38a-7a79-46d3-9a37-2b7bd0955810", "version": "24.01.000", "uri": "../flows/98daf38a-7a79-46d3-9a37-2b7bd0955810.xml"}, "exchange direction": "OUTPUT", "other": {"anies": [{"value": "0", "module": "A1-A3"}, {"name": "referenceToUnitGroupDataSet", "value": {"shortDescription": [{"value": "MJ", "lang": "en"}], "type": "unit group data set", "refObjectId": "93a60a57-a3c8-11da-a746-0800200c9a66", "version": "03.00.000", "uri": "../unitgroups/93a60a57-a3c8-11da-a746-0800200c9a66.xml"}}, {"value": "0", "module": "A4"}, {"value": "0", "module": "C1"}, {"value": "0", "module": "C2"}, {"value": "51.6848876667091", "module": "C3"}, {"value": "0", "module": "C4"}, {"value": "0", "module": "D"}]}, "resolvedFlowVersion": "38.00.000", "flowProperties": [], "typeOfFlow": "Other flow", "classification": {"classHierarchy": "Quantities / Environmental quantities / EPD EN 15804 / LCI indicators", "name": "GaBiCategories"}}]}, "LCIAResults": {"LCIAResult": [{"referenceToLCIAMethodDataSet": {"shortDescription": [{"value": "Climate change", "lang": "en"}, {"value": "Globales Erwärmungspotenzial - total (GWP-total)", "lang": "de"}], "type": "LCIA method data set", "refObjectId": "a7ea142a-9749-11ed-a8fc-0242ac120002", "version": "24.01.000", "uri": "../lciamethods/a7ea142a-9749-11ed-a8fc-0242ac120002.xml"}, "other": {"anies": [{"value": "3.96243476113229", "module": "A1-A3"}, {"value": "3.68382683505818", "module": "A4"}, {"value": "0.000527707094058251", "module": "C1"}, {"value": "1.80850587742408", "module": "C2"}, {"value": "12.1291394939941", "module": "C3"}, {"value": "68.4281829683237", "module": "C4"}, {"value": "-14.2712420925249", "module": "D"}, {"name": "referenceToUnitGroupDataSet", "value": {"shortDescription": [{"value": "kg CO2 eq.", "lang": "en"}], "type": "unit group data set", "refObjectId": "1ebf3012-d0db-4de2-aefd-ef30cedb0be1", "version": "25.00.000", "uri": "../unitgroups/1ebf3012-d0db-4de2-aefd-ef30cedb0be1.xml"}}]}}, {"referenceToLCIAMethodDataSet": {"shortDescription": [{"value": "Climate change-Fossil", "lang": "en"}, {"value": "Globales Erwärmungspotenzial - fossil (GWP-fossil)", "lang": "de"}], "type": "LCIA method data set", "refObjectId": "a7ea19c0-9749-11ed-a8fc-0242ac120002", "version": "24.01.000", "uri": "../lciamethods/a7ea19c0-9749-11ed-a8fc-0242ac120002.xml"}, "other": {"anies": [{"value": "53.9867039649347", "module": "A1-A3"}, {"value": "3.71660140109252", "module": "A4"}, {"value": "0.000514058862090979", "module": "C1"}, {"value": "1.76448716402581", "module": "C2"}, {"value": "12.1282897477353", "module": "C3"}, {"value": "12.7585808270099", "module": "C4"}, {"value": "-14.2525616333831", "module": "D"}, {"name": "referenceToUnitGroupDataSet", "value": {"shortDescription": [{"value": "kg CO2 eq.", "lang": "en"}], "type": "unit group data set", "refObjectId": "1ebf3012-d0db-4de2-aefd-ef30cedb0be1", "version": "25.00.000", "uri": "../unitgroups/1ebf3012-d0db-4de2-aefd-ef30cedb0be1.xml"}}]}}, {"referenceToLCIAMethodDataSet": {"shortDescription": [{"value": "Climate change-Biogenic", "lang": "en"}, {"value": "Globales Erwärmungspotenzial - biogen (GWP-biogenic)", "lang": "de"}], "type": "LCIA method data set", "refObjectId": "a7ea186c-9749-11ed-a8fc-0242ac120002", "version": "24.01.000", "uri": "../lciamethods/a7ea186c-9749-11ed-a8fc-0242ac120002.xml"}, "other": {"anies": [{"value": "-50.4863530172028", "module": "A1-A3"}, {"value": "-0.0942561722672039", "module": "A4"}, {"value": "3.69660976413491E-6", "module": "C1"}, {"value": "0.0100916704598027", "module": "C2"}, {"value": "0.000776432469543425", "module": "C3"}, {"value": "55.6261753715078", "module": "C4"}, {"value": "-0.00797820628552156", "module": "D"}, {"name": "referenceToUnitGroupDataSet", "value": {"shortDescription": [{"value": "kg CO2 eq.", "lang": "en"}], "type": "unit group data set", "refObjectId": "1ebf3012-d0db-4de2-aefd-ef30cedb0be1", "version": "25.00.000", "uri": "../unitgroups/1ebf3012-d0db-4de2-aefd-ef30cedb0be1.xml"}}]}}, {"referenceToLCIAMethodDataSet": {"shortDescription": [{"value": "Climate change-Land use and land use change", "lang": "en"}, {"value": "Globales Erwärmungspotenzial - luluc (GWP-luluc)", "lang": "de"}], "type": "LCIA method data set", "refObjectId": "a7ea1ae2-9749-11ed-a8fc-0242ac120002", "version": "24.01.000", "uri": "../lciamethods/a7ea1ae2-9749-11ed-a8fc-0242ac120002.xml"}, "other": {"anies": [{"value": "0.462083813400304", "module": "A1-A3"}, {"value": "0.0614816062328686", "module": "A4"}, {"value": "9.95162220313751E-6", "module": "C1"}, {"value": "0.0339270429384684", "module": "C2"}, {"value": "7.33137892630103E-5", "module": "C3"}, {"value": "0.0434267698060769", "module": "C4"}, {"value": "-0.0107022528562274", "module": "D"}, {"name": "referenceToUnitGroupDataSet", "value": {"shortDescription": [{"value": "kg CO2 eq.", "lang": "en"}], "type": "unit group data set", "refObjectId": "1ebf3012-d0db-4de2-aefd-ef30cedb0be1", "version": "25.00.000", "uri": "../unitgroups/1ebf3012-d0db-4de2-aefd-ef30cedb0be1.xml"}}]}}, {"referenceToLCIAMethodDataSet": {"shortDescription": [{"value": "Depletion potenzial of the stratospheric ozone layer (ODP)", "lang": "en"}, {"value": "Abbaupotenzial der stratosphärischen Ozonschicht (ODP)", "lang": "de"}], "type": "LCIA method data set", "refObjectId": "b5c629d6-def3-11e6-bf01-fe55135034f3", "version": "24.01.000", "uri": "../lciamethods/b5c629d6-def3-11e6-bf01-fe55135034f3.xml"}, "other": {"anies": [{"value": "1.31443502885054E-10", "module": "A1-A3"}, {"value": "3.68588291144211E-13", "module": "A4"}, {"value": "1.20888488153136E-16", "module": "C1"}, {"value": "5.56996702416832E-13", "module": "C2"}, {"value": "1.45225013603144E-12", "module": "C3"}, {"value": "2.86210208762225E-11", "module": "C4"}, {"value": "-9.75438640192394E-11", "module": "D"}, {"name": "referenceToUnitGroupDataSet", "value": {"shortDescription": [{"value": "kg CFC-11 eq.", "lang": "en"}], "type": "unit group data set", "refObjectId": "d9e957c9-7309-4474-bf3a-7777df6c4e5b", "version": "25.00.000", "uri": "../unitgroups/d9e957c9-7309-4474-bf3a-7777df6c4e5b.xml"}}]}}, {"referenceToLCIAMethodDataSet": {"shortDescription": [{"value": "Acidifcation potential, Accumulated Exceedance (AP)", "lang": "en"}, {"value": "Versauerungspotenzial, kumulierte Überschreitung (AP)", "lang": "de"}], "type": "LCIA method data set", "refObjectId": "b5c611c6-def3-11e6-bf01-fe55135034f3", "version": "24.01.000", "uri": "../lciamethods/b5c611c6-def3-11e6-bf01-fe55135034f3.xml"}, "other": {"anies": [{"value": "0.163934557540417", "module": "A1-A3"}, {"value": "0.00427481432842694", "module": "A4"}, {"value": "6.9508159119834E-6", "module": "C1"}, {"value": "0.00321340826845029", "module": "C2"}, {"value": "0.0017797692067974", "module": "C3"}, {"value": "0.0685100882365011", "module": "C4"}, {"value": "-0.0386223219191059", "module": "D"}, {"name": "referenceToUnitGroupDataSet", "value": {"shortDescription": [{"value": "Mole of H+ eq.", "lang": "en"}], "type": "unit group data set", "refObjectId": "42e089ac-92bf-4bf2-8ca1-5fc40d18f2ed", "version": "00.01.000", "uri": "../unitgroups/42e089ac-92bf-4bf2-8ca1-5fc40d18f2ed.xml"}}]}}, {"referenceToLCIAMethodDataSet": {"shortDescription": [{"value": "Eutrophication, freshwater", "lang": "en"}, {"value": "Eutrophierungspotenzial - Süßwasser (EP-freshwater)", "lang": "de"}], "type": "LCIA method data set", "refObjectId": "b53ec18f-7377-4ad3-86eb-cc3f4f276b2b", "version": "24.01.000", "uri": "../lciamethods/b53ec18f-7377-4ad3-86eb-cc3f4f276b2b.xml"}, "other": {"anies": [{"value": "0.000158091462108784", "module": "A1-A3"}, {"value": "1.56170761223E-5", "module": "A4"}, {"value": "1.39537941743943E-9", "module": "C1"}, {"value": "4.803343016689E-6", "module": "C2"}, {"value": "3.4678111434281E-7", "module": "C3"}, {"value": "0.00436177762229767", "module": "C4"}, {"value": "-1.94162818140134E-5", "module": "D"}, {"name": "referenceToUnitGroupDataSet", "value": {"shortDescription": [{"value": "kg P eq.", "lang": "en"}], "type": "unit group data set", "refObjectId": "0429039d-a61d-4590-ba67-aa4a20a810a1", "version": "25.00.000", "uri": "../unitgroups/0429039d-a61d-4590-ba67-aa4a20a810a1.xml"}}]}}, {"referenceToLCIAMethodDataSet": {"shortDescription": [{"value": "Eutrophication marine", "lang": "en"}, {"value": "Eutrophierungspotenzial - Salzwasser (EP-marine)", "lang": "de"}], "type": "LCIA method data set", "refObjectId": "b5c619fa-def3-11e6-bf01-fe55135034f3", "version": "24.01.000", "uri": "../lciamethods/b5c619fa-def3-11e6-bf01-fe55135034f3.xml"}, "other": {"anies": [{"value": "0.0447785041119887", "module": "A1-A3"}, {"value": "0.00143733167464169", "module": "A4"}, {"value": "3.1565176962515E-6", "module": "C1"}, {"value": "0.00129141663928517", "module": "C2"}, {"value": "0.000312509671557151", "module": "C3"}, {"value": "0.0482288924046321", "module": "C4"}, {"value": "-0.00703127545958353", "module": "D"}, {"name": "referenceToUnitGroupDataSet", "value": {"shortDescription": [{"value": "kg N eq.", "lang": "en"}], "type": "unit group data set", "refObjectId": "d05bb823-ecdf-4686-8c40-bf1d9257859f", "version": "00.00.003", "uri": "../unitgroups/d05bb823-ecdf-4686-8c40-bf1d9257859f.xml"}}]}}, {"referenceToLCIAMethodDataSet": {"shortDescription": [{"value": "Eutrophication, terrestrial", "lang": "en"}, {"value": "Eutrophierungspotenzial - Land (EP-terrestrial)", "lang": "de"}], "type": "LCIA method data set", "refObjectId": "b5c614d2-def3-11e6-bf01-fe55135034f3", "version": "24.01.000", "uri": "../lciamethods/b5c614d2-def3-11e6-bf01-fe55135034f3.xml"}, "other": {"anies": [{"value": "0.501300749887485", "module": "A1-A3"}, {"value": "0.0174708199770617", "module": "A4"}, {"value": "3.47827707672971E-5", "module": "C1"}, {"value": "0.0151222425908846", "module": "C2"}, {"value": "0.00834170339417824", "module": "C3"}, {"value": "0.20949984249869", "module": "C4"}, {"value": "-0.0767788216204161", "module": "D"}, {"name": "referenceToUnitGroupDataSet", "value": {"shortDescription": [{"value": "Mole of N eq.", "lang": "en"}], "type": "unit group data set", "refObjectId": "71b4d617-0ec9-4d3f-b65e-e438940c2401", "version": "00.00.003", "uri": "../unitgroups/71b4d617-0ec9-4d3f-b65e-e438940c2401.xml"}}]}}, {"referenceToLCIAMethodDataSet": {"shortDescription": [{"value": "Photochemical Ozone Creation Potential  (POCP)", "lang": "en"}, {"value": "Bildungspotenzial für troposphärisches Ozon (POCP)", "lang": "de"}], "type": "LCIA method data set", "refObjectId": "b5c610fe-def3-11e6-bf01-fe55135034f3", "version": "24.01.000", "uri": "../lciamethods/b5c610fe-def3-11e6-bf01-fe55135034f3.xml"}, "other": {"anies": [{"value": "0.134806228904652", "module": "A1-A3"}, {"value": "0.00402063723185518", "module": "A4"}, {"value": "9.49974020679331E-6", "module": "C1"}, {"value": "0.00308197600234776", "module": "C2"}, {"value": "0.00084524701606359", "module": "C3"}, {"value": "0.0839272936160958", "module": "C4"}, {"value": "-0.0214778140652165", "module": "D"}, {"name": "referenceToUnitGroupDataSet", "value": {"shortDescription": [{"value": "kg NMVOC eq.", "lang": "en"}], "type": "unit group data set", "refObjectId": "d27c25f8-fbc1-44c6-b47b-4adbae4199c6", "version": "00.00.003", "uri": "../unitgroups/d27c25f8-fbc1-44c6-b47b-4adbae4199c6.xml"}}]}}, {"referenceToLCIAMethodDataSet": {"shortDescription": [{"value": "Resource use, minerals and metals", "lang": "en"}, {"value": "Potenzial für die Verknappung abiotischer Ressourcen  nicht fossile Ressourcen (ADPE)", "lang": "de"}], "type": "LCIA method data set", "refObjectId": "b2ad6494-c78d-11e6-9d9d-cec0c932ce01", "version": "24.01.000", "uri": "../lciamethods/b2ad6494-c78d-11e6-9d9d-cec0c932ce01.xml"}, "other": {"anies": [{"value": "0.000478058410777527", "module": "A1-A3"}, {"value": "3.09437014423367E-7", "module": "A4"}, {"value": "8.75788060253732E-11", "module": "C1"}, {"value": "2.99330131229466E-7", "module": "C2"}, {"value": "1.15569623382113E-8", "module": "C3"}, {"value": "6.34118500805707E-7", "module": "C4"}, {"value": "-0.000118319955619278", "module": "D"}, {"name": "referenceToUnitGroupDataSet", "value": {"shortDescription": [{"value": "kg Sb eq.", "lang": "en"}], "type": "unit group data set", "refObjectId": "54ccd2d9-a32a-4fc2-923d-f2c8c93e89d4", "version": "25.00.000", "uri": "../unitgroups/54ccd2d9-a32a-4fc2-923d-f2c8c93e89d4.xml"}}]}}, {"referenceToLCIAMethodDataSet": {"shortDescription": [{"value": "Resource use, fossils", "lang": "en"}, {"value": "Potenzial für die Verknappung abiotischer Ressourcen  fossile Brennstoffe (ADPF)", "lang": "de"}], "type": "LCIA method data set", "refObjectId": "b2ad6110-c78d-11e6-9d9d-cec0c932ce01", "version": "24.01.000", "uri": "../lciamethods/b2ad6110-c78d-11e6-9d9d-cec0c932ce01.xml"}, "other": {"anies": [{"value": "1165.34908323023", "module": "A1-A3"}, {"value": "47.7569512557259", "module": "A4"}, {"value": "0.00674392792743425", "module": "C1"}, {"value": "23.1597029666374", "module": "C2"}, {"value": "1.97375240445628", "module": "C3"}, {"value": "177.794948877102", "module": "C4"}, {"value": "-169.745859775818", "module": "D"}, {"name": "referenceToUnitGroupDataSet", "value": {"shortDescription": [{"value": "MJ", "lang": "en"}], "type": "unit group data set", "refObjectId": "93a60a57-a3c8-11da-a746-0800200c9a66", "version": "02.00.000", "uri": "../unitgroups/93a60a57-a3c8-11da-a746-0800200c9a66.xml"}}]}}, {"referenceToLCIAMethodDataSet": {"shortDescription": [{"value": "Water use", "lang": "en"}, {"value": "Wasser-Entzugspotenzial (Benutzer) (WDP)", "lang": "de"}], "type": "LCIA method data set", "refObjectId": "b2ad66ce-c78d-11e6-9d9d-cec0c932ce01", "version": "24.01.000", "uri": "../lciamethods/b2ad66ce-c78d-11e6-9d9d-cec0c932ce01.xml"}, "other": {"anies": [{"value": "2.97946140569353", "module": "A1-A3"}, {"value": "0.0544901891607306", "module": "A4"}, {"value": "3.65348828197644E-6", "module": "C1"}, {"value": "0.0126425109914364", "module": "C2"}, {"value": "1.1663597563614", "module": "C3"}, {"value": "0.909075811129916", "module": "C4"}, {"value": "-1.66386901091634", "module": "D"}, {"name": "referenceToUnitGroupDataSet", "value": {"shortDescription": [{"value": "m³ world equiv.", "lang": "en"}], "type": "unit group data set", "refObjectId": "6ae2df01-888e-46c8-b17d-49fa3869b476", "version": "00.00.003", "uri": "../unitgroups/6ae2df01-888e-46c8-b17d-49fa3869b476.xml"}}]}}]}, "otherAttributes": {"{http://www.indata.network/EPD/2019}epd-version": "1.2"}, "version": "1.1", "locations": "../ILCDLocations.xml"}