{"processInformation": {"dataSetInformation": {"UUID": "432e4b39-301e-4154-ac8a-ac635d6c36ad", "name": {"baseName": [{"value": "Plastic profile EPDM", "lang": "en"}, {"value": "Kunststoffprofil EPDM", "lang": "de"}], "functionalUnitFlowProperties": [{"value": "EPDM", "lang": "en"}]}, "classificationInformation": {"classification": [{"class": [{"value": "Kunststoffe", "level": 0, "classId": "6"}, {"value": "Profile", "level": 1, "classId": "6.4"}, {"value": "Kunststoffprofile elastisch", "level": 2, "classId": "6.4.02"}], "name": "oekobau.dat"}]}, "generalComment": [{"value": "This data set has been modeled according to the European Standard EN 15804+A2 for Sustainable Building. Results are depicted in modules that allow the structured expression of results over the entire life cycle.", "lang": "en"}, {"value": "Dieser Datensatz wurde nach dem European Standard EN 15804+A2 für Nachhaltiges Bauen modelliert. Ergebnisse werden in Modulen abgebildet, die den strukturierten Ausdruck von Ergebnissen über den gesamten Lebenszyklus zulassen.", "lang": "de"}], "other": {"anies": [{"margins": 10, "description": [{"value": "Product system almost completely covered. Good technological, temporal and geographic representativeness.", "lang": "en"}, {"value": "Produktsystem weitgehend vollständig abgebildet. Gute technologische, zeitliche und geographische Repräsentativität.", "lang": "de"}]}]}}, "quantitativeReference": {"referenceToReferenceFlow": [101501], "type": "Reference flow(s)"}, "time": {"referenceYear": 2023, "dataSetValidUntil": 2026, "timeRepresentativenessDescription": [{"value": "Annual average", "lang": "en"}, {"value": "Jährlicher Durchschnitt", "lang": "de"}]}, "geography": {"locationOfOperationSupplyOrProduction": {"descriptionOfRestrictions": [{"value": "The data set represents the country specific situation in Germany, focusing on the main technologies, the region specific characteristics and / or import statistics.", "lang": "en"}, {"value": "Der Datensatz bildet die länderspezifische Situation in Deutschland ab. Dabei werden Haupttechnologien, spezifische regionale Charakteristiken und ggf. Importstatistiken berücksichtigt.", "lang": "de"}], "location": "DE"}}, "technology": {"technologyDescriptionAndIncludedProcesses": [{"value": "The life cycle analysis of the EPDM plastic profile includes the life cycle phases cradle to gate. The system boundary is the product (ready for sale). Transports from the factory to the mounting location are not taken into account and have to be incorporated in a system approach if necessary. EPDM production: EPDM is produced by the copolymerization of ethylene and propylene. The polymerization is carried out in solution. The process is run at 10- 50°C and 1- 20 bar in a single continuous stirred tank reactor, a catalyst is used. Because the polymerization is strongly exothermal, cooling is required. Organic solvents like hexane are used. Unreacted propene is recycled and reintroduced into the reactor. The solvent is also recovered. Downstream of the reactor, the reaction is shortstopped with water, alcohol or other polar liquids. The polymer solution is mixed with sodium hydroxide to remove catalyst residues. After adding chemicals like extender oil, the polymer solution is stripped with steam and hot water to remove unreacted monomers and solvents. Antiagglomerants and antifoaming agents may be added to control crumb agglomeration of the rubber product. The product is then passed over a screen and dried.\n\nIn module C1, a manual dismantling (no loads) is assumed, collecting losses are neglected.\nThe transport in module C2 to the recycling plant takes place with a truck (50km).\nModule C3 takes into account the grinding and thermal treatment (combustion) of the material. When calculating combustion emissions and credits, the specific calorific value of each material and the material composition are taken into account.\nIn module D credits for the substitution of electricity (German electricity mix) and thermal energy (from natural gas) are given.", "lang": "en"}, {"value": "Die Ökobilanzierung umfasst die Rohstoffbereitstellung, den Rohstofftransport und den Herstellungsaufwand für ein  EPDM-Kunststoffprofil sowie dessen Entsorgung. Transporte vom Werk zum Einbauort sind nicht berücksichtigt und sollten nach Bedarf nachträglich einbezogen werden.\nZur Herstellung von EPDM: EPDM entsteht aus der Co-Polymerisation von Ethylen und Propylen. Die Polymerisation findet in Lösung statt. Der Prozess erfolgt bei Temperaturen zwischen 10 und 50°C und Druckverhältnissen zwischen 1  und 20 bar in einem kontinuierlichen Rührtankreaktor unter Zugabe eines Katalysators. Die Reaktion ist stark exotherm, was eine Kühlung notwendig macht. Organische Lösungsmittel wie Hexan kommen zum Einsatz. Nicht umgesetztes Propylen wird recycelt und wieder in den Reaktor eingespeist. Dem Reaktor nachgeschaltet erfolgt das Abstoppen der Reaktion mit Hilfe von Wasser, Alkohol oder anderen polaren Flüssigkeiten. Anschließend wird die Polymerlösung mit Natriumhydroxid gemischt, um die verbliebenen Katalysatorreste zu entfernen. Extenderöl oder ähnliche Substanzen werden zugegeben. Danach wird die Polymerlösung mit Dampf und heißem Wasser behandelt, um nicht umgesetzte Monomere und restliches Lösungsmittel zu beseitigen. Zur Sicherstellung einer kontrollierten Ausflockung werden Entschäumer und Trennmittel zugegeben.  Anschließend erfolgt die Trocknung. \n\nIn Modul C1 wird ein manueller Rückbau (lastenfrei) angenommen. Sammelverluste werden vernachlässigt.\nDer Transport in Modul C2 zur Verwertungsanlage erfolgt mit einem LKW (50km). \nIn Modul C3 wird die Zerkleinerung und thermische Behandlung (Verbrennung) des Materials berücksichtigt. Bei der Berechnung der Verbrennungsemissionen und Gutschriften wird der spezifische Heizwert des jeweiligen Materials sowie die Materialzusammensetzung berücksichtigt.\nIn Modul D erfolgen Gutschriften für die Substitution von Strom (deutscher Strommix) und thermischer Energie (aus Erdgas).", "lang": "de"}], "technologicalApplicability": [{"value": "This product can be used in construction.", "lang": "en"}, {"value": "Dieses Produkt kann im Baubereich verwendet werden.", "lang": "de"}], "referenceToTechnologyFlowDiagrammOrPicture": [{"shortDescription": [{"value": "construction_de_plastic profile epdm.jpg", "lang": "en"}], "type": "source data set", "refObjectId": "e5bc3dc5-d2c2-44be-a883-4a29cc1bfb6a", "version": "24.01.000", "uri": "../sources/e5bc3dc5-d2c2-44be-a883-4a29cc1bfb6a.xml"}]}}, "modellingAndValidation": {"LCIMethodAndAllocation": {"typeOfDataSet": "EPD", "other": {"anies": [{"name": "subType", "value": "generic dataset"}]}}, "dataSourcesTreatmentAndRepresentativeness": {"referenceToDataSource": [{"shortDescription": [{"value": "Plastics Europe Association of Plastics Manufacturers, 2006", "lang": "en"}], "type": "source data set", "refObjectId": "ef0ac214-84b1-45e5-b271-7ef9e66d5fd8", "version": "24.01.000", "uri": "../sources/ef0ac214-84b1-45e5-b271-7ef9e66d5fd8.xml"}, {"shortDescription": [{"value": "ULLMANN'S Encyclopedia of Industrial Chemistry 1999-2023", "lang": "en"}], "type": "source data set", "refObjectId": "d2732231-5fbd-11db-b0de-0800200c9a66", "version": "24.01.000", "uri": "../sources/d2732231-5fbd-11db-b0de-0800200c9a66.xml"}, {"shortDescription": [{"value": "Documentation of data quality management", "lang": "en"}], "type": "source data set", "refObjectId": "e3bd9bbf-2c3c-42aa-8892-fd13f1065ca5", "version": "24.01.000", "uri": "../sources/e3bd9bbf-2c3c-42aa-8892-fd13f1065ca5.xml"}, {"shortDescription": [{"value": "GaBi Database Edition 2021, CUP2021.01", "lang": "en"}], "type": "source data set", "refObjectId": "1cece811-7501-44d4-8067-9259bd5cb835", "version": "00.01.000", "uri": "../sources/1cece811-7501-44d4-8067-9259bd5cb835.xml"}, {"shortDescription": [{"value": "Sphera Managed LCA Content Databases (all versions)", "lang": "en"}], "type": "source data set", "refObjectId": "28d74cc0-db8b-4d7e-bc44-5f6d56ce0c4a", "version": "00.03.002", "uri": "../sources/28d74cc0-db8b-4d7e-bc44-5f6d56ce0c4a.xml"}], "useAdviceForDataSet": [{"value": "The data set represents a cradle to gate inventory. It can be used to characterise the supply chain situation of the respective commodity in a representative manner. Combination with individual unit processes using this commodity enables the generation of user-specific (product) LCAs.", "lang": "en"}, {"value": "Der Datensatz repräsentiert ein Cradle to Gate Inventar. Er kann verwendet werden, um die Lieferkette des jeweiligen Produktes in einer repräsentativen Weise zu charakterisieren. Die Kombination mit einzelnen Einheitenprozessen und diesem Produkt ermöglicht die Erstellung von anwenderspezifischen (Produkt-) LCAs.", "lang": "de"}]}, "validation": {"review": [{"referenceToNameOfReviewerAndInstitution": [{"shortDescription": [{"value": "Sphera Solutions GmbH", "lang": "en"}], "type": "contact data set", "refObjectId": "d7fa0337-f279-430d-becf-7f3111a85010", "version": "24.01.000", "uri": "../contacts/d7fa0337-f279-430d-becf-7f3111a85010.xml"}], "type": "Dependent internal review"}, {"referenceToNameOfReviewerAndInstitution": [{"shortDescription": [{"value": "Sphera Product Sustainability user forum", "lang": "en"}], "type": "contact data set", "refObjectId": "8f1306f0-7b83-4f36-a537-aa83f0498266", "version": "24.01.000", "uri": "../contacts/8f1306f0-7b83-4f36-a537-aa83f0498266.xml"}], "type": "Independent external review"}]}, "complianceDeclarations": {"compliance": [{"referenceToComplianceSystem": {"shortDescription": [{"value": "EN 15804+A2 (EF 3.1)", "lang": "de"}, {"value": "EN 15804+A2 (EF 3.1)", "lang": "en"}], "type": "source data set", "refObjectId": "d4aa3ec7-b1d7-4a4a-a6cb-37af88dcc902", "version": "00.01.000", "uri": "../sources/d4aa3ec7-b1d7-4a4a-a6cb-37af88dcc902.xml"}, "approvalOfOverallCompliance": "Fully compliant"}]}}, "administrativeInformation": {"dataGenerator": {"referenceToPersonOrEntityGeneratingTheDataSet": [{"shortDescription": [{"value": "Sphera Solutions GmbH", "lang": "en"}], "type": "contact data set", "refObjectId": "d7fa0337-f279-430d-becf-7f3111a85010", "version": "24.01.000", "uri": "../contacts/d7fa0337-f279-430d-becf-7f3111a85010.xml"}]}, "dataEntryBy": {"timeStamp": 1718121663000, "referenceToDataSetFormat": [{"shortDescription": [{"value": "ILCD format 1.1", "lang": "de"}, {"value": "ILCD format 1.1", "lang": "en"}], "type": "source data set", "refObjectId": "a97a0155-0234-4b87-b4ce-a45da52f2a40", "version": "01.00.000", "uri": "../sources/a97a0155-0234-4b87-b4ce-a45da52f2a40.xml"}, {"shortDescription": [{"value": "EPD-Datenformaterweiterungen v1.2", "lang": "de"}, {"value": "EPD Data Format Extensions v1.2", "lang": "en"}], "type": "source data set", "refObjectId": "a29449fd-aa2f-4de8-b5d7-4b06b43c6fde", "version": "00.01.000", "uri": "../sources/a29449fd-aa2f-4de8-b5d7-4b06b43c6fde.xml"}], "referenceToPersonOrEntityEnteringTheData": {"shortDescription": [{"value": "Sphera Solutions GmbH", "lang": "en"}], "type": "contact data set", "refObjectId": "d7fa0337-f279-430d-becf-7f3111a85010", "version": "24.01.000", "uri": "../contacts/d7fa0337-f279-430d-becf-7f3111a85010.xml"}}, "publicationAndOwnership": {"dataSetVersion": "20.24.070", "referenceToPrecedingDataSetVersion": [{"shortDescription": [{"value": "Plastic profile EPDM", "lang": "en"}], "type": "process data set", "refObjectId": "963ffb34-439a-4cab-9bfb-28c9b42533f2", "uri": "https://www.oekobaudat.de/OEKOBAU.DAT/resource/processes/963ffb34-439a-4cab-9bfb-28c9b42533f2?version=20.23.050"}], "referenceToRegistrationAuthority": {"shortDescription": [{"value": "Sphera Solutions GmbH", "lang": "en"}], "type": "contact data set", "refObjectId": "d7fa0337-f279-430d-becf-7f3111a85010", "version": "24.01.000", "uri": "../contacts/d7fa0337-f279-430d-becf-7f3111a85010.xml"}, "referenceToOwnershipOfDataSet": {"shortDescription": [{"value": "Sphera Solutions GmbH", "lang": "en"}], "type": "contact data set", "refObjectId": "d7fa0337-f279-430d-becf-7f3111a85010", "version": "24.01.000", "uri": "../contacts/d7fa0337-f279-430d-becf-7f3111a85010.xml"}, "copyright": true, "licenseType": "Free of charge for all users and uses", "accessRestrictions": [{"value": "The license conditions as stated on https://www.oekobaudat.de/apply.", "lang": "en"}, {"value": "Es gelten die Lizenzbedingungen wie sie auf https://www.oekobaudat.de/ genannt sind.", "lang": "de"}], "other": {"anies": [{"name": "referenceToPublisher", "value": {"shortDescription": [{"value": "BBSR", "lang": "en"}], "type": "contact data set", "refObjectId": "f11651e0-7877-11e3-981f-0800200c9a66", "version": "00.01.000", "uri": "../contacts/f11651e0-7877-11e3-981f-0800200c9a66.xml"}}]}}}, "exchanges": {"exchange": [{"dataSetInternalID": 101501, "referenceToFlowDataSet": {"shortDescription": [{"value": "Plastic profile EPDM", "lang": "en"}, {"value": "Kunststoffprofil EPDM", "lang": "de"}], "type": "flow data set", "refObjectId": "2b71cca2-228b-429a-b2f8-fac20a8e0cff", "version": "24.01.000", "uri": "../flows/2b71cca2-228b-429a-b2f8-fac20a8e0cff.xml"}, "meanAmount": 1.0, "referenceFlow": true, "resultingflowAmount": 1.0, "flowProperties": [{"name": [{"lang": "en", "value": "Mass"}, {"lang": "de", "value": "Masse"}], "uuid": "93a60a56-a3c8-11da-a746-0800200b9a66", "referenceFlowProperty": true, "meanValue": 1.0, "referenceUnit": "kg", "unitGroupUUID": "ad38d542-3fe9-439d-9b95-2f5f7752acaf"}], "materialProperties": [{"name": "gross density", "value": "400.0", "unit": "kg/m^3", "unitDescription": "kilograms per cubic metre"}], "typeOfFlow": "Product flow", "classification": {"classHierarchy": "Valuable substances / Systems / Parts / Plastic parts", "name": "GaBiCategories"}}, {"dataSetInternalID": 101502, "referenceToFlowDataSet": {"shortDescription": [{"value": "Use of renewable primary energy as energy carrier (PERE)", "lang": "en"}, {"value": "Erneuerbare Primärenergie als Energieträger (PERE)", "lang": "de"}], "type": "flow data set", "refObjectId": "20f32be5-0398-4288-9b6d-accddd195317", "version": "24.01.000", "uri": "../flows/20f32be5-0398-4288-9b6d-accddd195317.xml"}, "exchange direction": "INPUT", "other": {"anies": [{"value": "10.8833354010844", "module": "A1-A3"}, {"name": "referenceToUnitGroupDataSet", "value": {"shortDescription": [{"value": "MJ", "lang": "en"}], "type": "unit group data set", "refObjectId": "93a60a57-a3c8-11da-a746-0800200c9a66", "version": "03.00.000", "uri": "../unitgroups/93a60a57-a3c8-11da-a746-0800200c9a66.xml"}}, {"value": "0.00483305291038269", "module": "C2"}, {"value": "0.198375003968686", "module": "C3"}, {"value": "-9.34845794692325", "module": "D"}]}, "resolvedFlowVersion": "38.00.000", "flowProperties": [], "typeOfFlow": "Other flow", "classification": {"classHierarchy": "Quantities", "name": "GaBiCategories"}}, {"dataSetInternalID": 101503, "referenceToFlowDataSet": {"shortDescription": [{"value": "Use of renewable primary energy resources used as raw materials (PERM)", "lang": "en"}, {"value": "Erneuerbare Primärenergie zur stofflichen Nutzung (PERM)", "lang": "de"}], "type": "flow data set", "refObjectId": "fb3ec0de-548d-4508-aea5-00b73bf6f702", "version": "24.01.000", "uri": "../flows/fb3ec0de-548d-4508-aea5-00b73bf6f702.xml"}, "exchange direction": "INPUT", "other": {"anies": [{"value": "0", "module": "A1-A3"}, {"name": "referenceToUnitGroupDataSet", "value": {"shortDescription": [{"value": "MJ", "lang": "en"}], "type": "unit group data set", "refObjectId": "93a60a57-a3c8-11da-a746-0800200c9a66", "version": "03.00.000", "uri": "../unitgroups/93a60a57-a3c8-11da-a746-0800200c9a66.xml"}}, {"value": "0", "module": "C2"}, {"value": "0", "module": "C3"}, {"value": "0", "module": "D"}]}, "resolvedFlowVersion": "38.00.000", "flowProperties": [], "typeOfFlow": "Other flow", "classification": {"classHierarchy": "Quantities", "name": "GaBiCategories"}}, {"dataSetInternalID": 101504, "referenceToFlowDataSet": {"shortDescription": [{"value": "Total use of renewable primary energy (PERT)", "lang": "en"}, {"value": "Total erneuerbare Primärenergie (PERT)", "lang": "de"}], "type": "flow data set", "refObjectId": "53f97275-fa8a-4cdd-9024-65936002acd0", "version": "24.01.000", "uri": "../flows/53f97275-fa8a-4cdd-9024-65936002acd0.xml"}, "exchange direction": "INPUT", "other": {"anies": [{"value": "10.8833354010844", "module": "A1-A3"}, {"name": "referenceToUnitGroupDataSet", "value": {"shortDescription": [{"value": "MJ", "lang": "en"}], "type": "unit group data set", "refObjectId": "93a60a57-a3c8-11da-a746-0800200c9a66", "version": "03.00.000", "uri": "../unitgroups/93a60a57-a3c8-11da-a746-0800200c9a66.xml"}}, {"value": "0.00483305291038269", "module": "C2"}, {"value": "0.198375003968686", "module": "C3"}, {"value": "-9.34845794692325", "module": "D"}]}, "resolvedFlowVersion": "38.00.000", "flowProperties": [], "typeOfFlow": "Other flow", "classification": {"classHierarchy": "Quantities / Environmental quantities / EPD EN 15804 / LCI indicators", "name": "GaBiCategories"}}, {"dataSetInternalID": 101505, "referenceToFlowDataSet": {"shortDescription": [{"value": "Use of non renewable primary energy as energy carrier (PENRE)", "lang": "en"}, {"value": "Nicht-erneuerbare Primärenergie als Energieträger (PENRE)", "lang": "de"}], "type": "flow data set", "refObjectId": "ac857178-2b45-46ec-892a-a9a4332f0372", "version": "24.01.000", "uri": "../flows/ac857178-2b45-46ec-892a-a9a4332f0372.xml"}, "exchange direction": "INPUT", "other": {"anies": [{"value": "63.3532570143671", "module": "A1-A3"}, {"name": "referenceToUnitGroupDataSet", "value": {"shortDescription": [{"value": "MJ", "lang": "en"}], "type": "unit group data set", "refObjectId": "93a60a57-a3c8-11da-a746-0800200c9a66", "version": "03.00.000", "uri": "../unitgroups/93a60a57-a3c8-11da-a746-0800200c9a66.xml"}}, {"value": "0.0436718393101385", "module": "C2"}, {"value": "47.8247553445901", "module": "C3"}, {"value": "-21.1648517381654", "module": "D"}]}, "resolvedFlowVersion": "38.00.000", "flowProperties": [], "typeOfFlow": "Other flow", "classification": {"classHierarchy": "Quantities", "name": "GaBiCategories"}}, {"dataSetInternalID": 101506, "referenceToFlowDataSet": {"shortDescription": [{"value": "Use of non renewable primary energy resources used as raw materials (PENRM)", "lang": "en"}, {"value": "Nicht-erneuerbare Primärenergie zur stofflichen Nutzung (PENRM)", "lang": "de"}], "type": "flow data set", "refObjectId": "1421caa0-679d-4bf4-b282-0eb850ccae27", "version": "24.01.000", "uri": "../flows/1421caa0-679d-4bf4-b282-0eb850ccae27.xml"}, "exchange direction": "INPUT", "other": {"anies": [{"value": "43", "module": "A1-A3"}, {"name": "referenceToUnitGroupDataSet", "value": {"shortDescription": [{"value": "MJ", "lang": "en"}], "type": "unit group data set", "refObjectId": "93a60a57-a3c8-11da-a746-0800200c9a66", "version": "03.00.000", "uri": "../unitgroups/93a60a57-a3c8-11da-a746-0800200c9a66.xml"}}, {"value": "0", "module": "C2"}, {"value": "-43", "module": "C3"}, {"value": "0", "module": "D"}]}, "resolvedFlowVersion": "38.00.000", "flowProperties": [], "typeOfFlow": "Other flow", "classification": {"classHierarchy": "Quantities", "name": "GaBiCategories"}}, {"dataSetInternalID": 101507, "referenceToFlowDataSet": {"shortDescription": [{"value": "Total use of non renewable primary energy resource (PENRT)", "lang": "en"}, {"value": "Total nicht-erneuerbare Primärenergie (PENRT)", "lang": "de"}], "type": "flow data set", "refObjectId": "06159210-646b-4c8d-8583-da9b3b95a6c1", "version": "24.01.000", "uri": "../flows/06159210-646b-4c8d-8583-da9b3b95a6c1.xml"}, "exchange direction": "INPUT", "other": {"anies": [{"value": "106.353257014367", "module": "A1-A3"}, {"name": "referenceToUnitGroupDataSet", "value": {"shortDescription": [{"value": "MJ", "lang": "en"}], "type": "unit group data set", "refObjectId": "93a60a57-a3c8-11da-a746-0800200c9a66", "version": "03.00.000", "uri": "../unitgroups/93a60a57-a3c8-11da-a746-0800200c9a66.xml"}}, {"value": "0.0436718393101385", "module": "C2"}, {"value": "4.82475534459013", "module": "C3"}, {"value": "-21.1648517381654", "module": "D"}]}, "resolvedFlowVersion": "38.00.000", "flowProperties": [], "typeOfFlow": "Other flow", "classification": {"classHierarchy": "Quantities / Environmental quantities / EPD EN 15804 / LCI indicators", "name": "GaBiCategories"}}, {"dataSetInternalID": 101508, "referenceToFlowDataSet": {"shortDescription": [{"value": "Use of secondary material (SM)", "lang": "en"}, {"value": "Einsatz von Sekundärstoffen (SM)", "lang": "de"}], "type": "flow data set", "refObjectId": "c6a1f35f-2d09-4f54-8dfb-97e502e1ce92", "version": "24.01.000", "uri": "../flows/c6a1f35f-2d09-4f54-8dfb-97e502e1ce92.xml"}, "exchange direction": "INPUT", "other": {"anies": [{"value": "0", "module": "A1-A3"}, {"name": "referenceToUnitGroupDataSet", "value": {"shortDescription": [{"value": "kg", "lang": "en"}], "type": "unit group data set", "refObjectId": "93a60a57-a4c8-11da-a746-0800200c9a66", "version": "03.00.000", "uri": "../unitgroups/93a60a57-a4c8-11da-a746-0800200c9a66.xml"}}, {"value": "0", "module": "C2"}, {"value": "0", "module": "C3"}, {"value": "0", "module": "D"}]}, "resolvedFlowVersion": "38.00.000", "flowProperties": [], "typeOfFlow": "Other flow", "classification": {"classHierarchy": "Quantities / Environmental quantities / EPD EN 15804 / LCI indicators", "name": "GaBiCategories"}}, {"dataSetInternalID": 101509, "referenceToFlowDataSet": {"shortDescription": [{"value": "Use of renewable secondary fuels (SF)", "lang": "en"}, {"value": "Erneuerbare Sekundärbrennstoffe (SF)", "lang": "de"}], "type": "flow data set", "refObjectId": "64333088-a55f-4aa2-9a31-c10b07816787", "version": "24.01.000", "uri": "../flows/64333088-a55f-4aa2-9a31-c10b07816787.xml"}, "exchange direction": "INPUT", "other": {"anies": [{"value": "0", "module": "A1-A3"}, {"name": "referenceToUnitGroupDataSet", "value": {"shortDescription": [{"value": "MJ", "lang": "en"}], "type": "unit group data set", "refObjectId": "93a60a57-a3c8-11da-a746-0800200c9a66", "version": "03.00.000", "uri": "../unitgroups/93a60a57-a3c8-11da-a746-0800200c9a66.xml"}}, {"value": "0", "module": "C2"}, {"value": "0", "module": "C3"}, {"value": "0", "module": "D"}]}, "resolvedFlowVersion": "38.00.000", "flowProperties": [], "typeOfFlow": "Other flow", "classification": {"classHierarchy": "Quantities / Environmental quantities / EPD EN 15804 / LCI indicators", "name": "GaBiCategories"}}, {"dataSetInternalID": 101510, "referenceToFlowDataSet": {"shortDescription": [{"value": "Use of non renewable secondary fuels (NRSF)", "lang": "en"}, {"value": "Nicht erneuerbare Sekundärbrennstoffe (NRSF)", "lang": "de"}], "type": "flow data set", "refObjectId": "89def144-d39a-4287-b86f-efde453ddcb2", "version": "24.01.000", "uri": "../flows/89def144-d39a-4287-b86f-efde453ddcb2.xml"}, "exchange direction": "INPUT", "other": {"anies": [{"value": "0", "module": "A1-A3"}, {"name": "referenceToUnitGroupDataSet", "value": {"shortDescription": [{"value": "MJ", "lang": "en"}], "type": "unit group data set", "refObjectId": "93a60a57-a3c8-11da-a746-0800200c9a66", "version": "03.00.000", "uri": "../unitgroups/93a60a57-a3c8-11da-a746-0800200c9a66.xml"}}, {"value": "0", "module": "C2"}, {"value": "0", "module": "C3"}, {"value": "0", "module": "D"}]}, "resolvedFlowVersion": "38.00.000", "flowProperties": [], "typeOfFlow": "Other flow", "classification": {"classHierarchy": "Quantities / Environmental quantities / EPD EN 15804 / LCI indicators", "name": "GaBiCategories"}}, {"dataSetInternalID": 101511, "referenceToFlowDataSet": {"shortDescription": [{"value": "Net use of fresh water (FW)", "lang": "en"}, {"value": "Nettoeinsatz von Süßwasserressourcen (FW)", "lang": "de"}], "type": "flow data set", "refObjectId": "3cf952c8-f3a4-461d-8c96-96456ca62246", "version": "24.01.000", "uri": "../flows/3cf952c8-f3a4-461d-8c96-96456ca62246.xml"}, "exchange direction": "INPUT", "other": {"anies": [{"value": "0.0136445642559587", "module": "A1-A3"}, {"name": "referenceToUnitGroupDataSet", "value": {"shortDescription": [{"value": "m3", "lang": "en"}], "type": "unit group data set", "refObjectId": "93a60a57-a3c8-12da-a746-0800200c9a66", "version": "03.00.000", "uri": "../unitgroups/93a60a57-a3c8-12da-a746-0800200c9a66.xml"}}, {"value": "4.51511559639581E-6", "module": "C2"}, {"value": "0.00738023218232744", "module": "C3"}, {"value": "-0.00285838692015576", "module": "D"}]}, "resolvedFlowVersion": "38.00.000", "flowProperties": [], "typeOfFlow": "Other flow", "classification": {"classHierarchy": "Quantities / Environmental quantities / EPD EN 15804 / LCI indicators", "name": "GaBiCategories"}}, {"dataSetInternalID": 101512, "referenceToFlowDataSet": {"shortDescription": [{"value": "Hazardous waste disposed (HWD)", "lang": "en"}, {"value": "Gefährlicher Abfall zur Deponie (HWD)", "lang": "de"}], "type": "flow data set", "refObjectId": "430f9e0f-59b2-46a0-8e0d-55e0e84948fc", "version": "24.01.000", "uri": "../flows/430f9e0f-59b2-46a0-8e0d-55e0e84948fc.xml"}, "exchange direction": "OUTPUT", "other": {"anies": [{"value": "3.02093195380871E-8", "module": "A1-A3"}, {"name": "referenceToUnitGroupDataSet", "value": {"shortDescription": [{"value": "kg", "lang": "en"}], "type": "unit group data set", "refObjectId": "93a60a57-a4c8-11da-a746-0800200c9a66", "version": "03.00.000", "uri": "../unitgroups/93a60a57-a4c8-11da-a746-0800200c9a66.xml"}}, {"value": "2.12612433448568E-12", "module": "C2"}, {"value": "4.51368969897495E-10", "module": "C3"}, {"value": "-1.99371413703617E-8", "module": "D"}]}, "resolvedFlowVersion": "38.00.000", "flowProperties": [], "typeOfFlow": "Other flow", "classification": {"classHierarchy": "Quantities / Environmental quantities / EPD EN 15804 / LCI indicators", "name": "GaBiCategories"}}, {"dataSetInternalID": 101513, "referenceToFlowDataSet": {"shortDescription": [{"value": "Non harzardous waste disposed (NHWD)", "lang": "en"}, {"value": "Entsorgter nicht gefährlicher Abfall (NHWD)", "lang": "de"}], "type": "flow data set", "refObjectId": "b29ef66b-e286-4afa-949f-62f1a7b4d7fa", "version": "24.01.000", "uri": "../flows/b29ef66b-e286-4afa-949f-62f1a7b4d7fa.xml"}, "exchange direction": "OUTPUT", "other": {"anies": [{"value": "0.0665496703862492", "module": "A1-A3"}, {"name": "referenceToUnitGroupDataSet", "value": {"shortDescription": [{"value": "kg", "lang": "en"}], "type": "unit group data set", "refObjectId": "93a60a57-a4c8-11da-a746-0800200c9a66", "version": "03.00.000", "uri": "../unitgroups/93a60a57-a4c8-11da-a746-0800200c9a66.xml"}}, {"value": "7.38392325154112E-6", "module": "C2"}, {"value": "0.0374207480411175", "module": "C3"}, {"value": "-0.0126957079594399", "module": "D"}]}, "resolvedFlowVersion": "38.00.000", "flowProperties": [], "typeOfFlow": "Other flow", "classification": {"classHierarchy": "Quantities / Environmental quantities / EPD EN 15804 / LCI indicators", "name": "GaBiCategories"}}, {"dataSetInternalID": 101514, "referenceToFlowDataSet": {"shortDescription": [{"value": "Radioactive waste disposed (RWD)", "lang": "en"}, {"value": "Entsorgter radioaktiver Abfall (RWD)", "lang": "de"}], "type": "flow data set", "refObjectId": "3449546e-52ad-4b39-b809-9fb77cea8ff6", "version": "24.01.000", "uri": "../flows/3449546e-52ad-4b39-b809-9fb77cea8ff6.xml"}, "exchange direction": "OUTPUT", "other": {"anies": [{"value": "0.000982680749964308", "module": "A1-A3"}, {"name": "referenceToUnitGroupDataSet", "value": {"shortDescription": [{"value": "kg", "lang": "en"}], "type": "unit group data set", "refObjectId": "93a60a57-a4c8-11da-a746-0800200c9a66", "version": "03.00.000", "uri": "../unitgroups/93a60a57-a4c8-11da-a746-0800200c9a66.xml"}}, {"value": "6.95110807678198E-8", "module": "C2"}, {"value": "1.68342733105827E-5", "module": "C3"}, {"value": "-0.000505817683310926", "module": "D"}]}, "resolvedFlowVersion": "38.00.000", "flowProperties": [], "typeOfFlow": "Other flow", "classification": {"classHierarchy": "Quantities / Environmental quantities / EPD EN 15804 / LCI indicators", "name": "GaBiCategories"}}, {"dataSetInternalID": 101515, "referenceToFlowDataSet": {"shortDescription": [{"value": "Components for re-use (CRU)", "lang": "en"}, {"value": "Komponenten für die Wiederverwendung (CRU)", "lang": "de"}], "type": "flow data set", "refObjectId": "a2b32f97-3fc7-4af2-b209-525bc6426f33", "version": "24.01.000", "uri": "../flows/a2b32f97-3fc7-4af2-b209-525bc6426f33.xml"}, "exchange direction": "OUTPUT", "other": {"anies": [{"value": "0", "module": "A1-A3"}, {"name": "referenceToUnitGroupDataSet", "value": {"shortDescription": [{"value": "kg", "lang": "en"}], "type": "unit group data set", "refObjectId": "93a60a57-a4c8-11da-a746-0800200c9a66", "version": "03.00.000", "uri": "../unitgroups/93a60a57-a4c8-11da-a746-0800200c9a66.xml"}}, {"value": "0", "module": "C2"}, {"value": "0", "module": "C3"}, {"value": "0", "module": "D"}]}, "resolvedFlowVersion": "38.00.000", "flowProperties": [], "typeOfFlow": "Other flow", "classification": {"classHierarchy": "Quantities / Environmental quantities / EPD EN 15804 / LCI indicators", "name": "GaBiCategories"}}, {"dataSetInternalID": 101516, "referenceToFlowDataSet": {"shortDescription": [{"value": "Materials for recycling  (MFR)", "lang": "en"}, {"value": "Stoffe zum Recycling (MFR)", "lang": "de"}], "type": "flow data set", "refObjectId": "d7fe48a5-4103-49c8-9aae-b0b5dfdbd6ae", "version": "24.01.000", "uri": "../flows/d7fe48a5-4103-49c8-9aae-b0b5dfdbd6ae.xml"}, "exchange direction": "OUTPUT", "other": {"anies": [{"value": "0", "module": "A1-A3"}, {"name": "referenceToUnitGroupDataSet", "value": {"shortDescription": [{"value": "kg", "lang": "en"}], "type": "unit group data set", "refObjectId": "93a60a57-a4c8-11da-a746-0800200c9a66", "version": "03.00.000", "uri": "../unitgroups/93a60a57-a4c8-11da-a746-0800200c9a66.xml"}}, {"value": "0", "module": "C2"}, {"value": "0", "module": "C3"}, {"value": "0", "module": "D"}]}, "resolvedFlowVersion": "38.00.000", "flowProperties": [], "typeOfFlow": "Other flow", "classification": {"classHierarchy": "Quantities / Environmental quantities / EPD EN 15804 / LCI indicators", "name": "GaBiCategories"}}, {"dataSetInternalID": 101517, "referenceToFlowDataSet": {"shortDescription": [{"value": "Materials for energy recovery (MER)", "lang": "en"}, {"value": "Stoffe für die Energierückgewinnung (MER)", "lang": "de"}], "type": "flow data set", "refObjectId": "59a9181c-3aaf-46ee-8b13-2b3723b6e447", "version": "24.01.000", "uri": "../flows/59a9181c-3aaf-46ee-8b13-2b3723b6e447.xml"}, "exchange direction": "OUTPUT", "other": {"anies": [{"value": "0", "module": "A1-A3"}, {"name": "referenceToUnitGroupDataSet", "value": {"shortDescription": [{"value": "kg", "lang": "en"}], "type": "unit group data set", "refObjectId": "93a60a57-a4c8-11da-a746-0800200c9a66", "version": "03.00.000", "uri": "../unitgroups/93a60a57-a4c8-11da-a746-0800200c9a66.xml"}}, {"value": "0", "module": "C2"}, {"value": "0", "module": "C3"}, {"value": "0", "module": "D"}]}, "resolvedFlowVersion": "38.00.000", "flowProperties": [], "typeOfFlow": "Other flow", "classification": {"classHierarchy": "Quantities / Environmental quantities / EPD EN 15804 / LCI indicators", "name": "GaBiCategories"}}, {"dataSetInternalID": 101518, "referenceToFlowDataSet": {"shortDescription": [{"value": "Exported electrical energy (EEE)", "lang": "en"}, {"value": "Exportierte elektrische Energie (EEE)", "lang": "de"}], "type": "flow data set", "refObjectId": "4da0c987-2b76-40d6-9e9e-82a017aaaf29", "version": "24.01.000", "uri": "../flows/4da0c987-2b76-40d6-9e9e-82a017aaaf29.xml"}, "exchange direction": "OUTPUT", "other": {"anies": [{"value": "0", "module": "A1-A3"}, {"name": "referenceToUnitGroupDataSet", "value": {"shortDescription": [{"value": "MJ", "lang": "en"}], "type": "unit group data set", "refObjectId": "93a60a57-a3c8-11da-a746-0800200c9a66", "version": "03.00.000", "uri": "../unitgroups/93a60a57-a3c8-11da-a746-0800200c9a66.xml"}}, {"value": "0", "module": "C2"}, {"value": "5.7015310328053", "module": "C3"}, {"value": "0", "module": "D"}]}, "resolvedFlowVersion": "38.00.000", "flowProperties": [], "typeOfFlow": "Other flow", "classification": {"classHierarchy": "Quantities / Environmental quantities / EPD EN 15804 / LCI indicators", "name": "GaBiCategories"}}, {"dataSetInternalID": 101519, "referenceToFlowDataSet": {"shortDescription": [{"value": "Exported thermal energy (EET)", "lang": "en"}, {"value": "Exportierte thermische Energie (EET)", "lang": "de"}], "type": "flow data set", "refObjectId": "98daf38a-7a79-46d3-9a37-2b7bd0955810", "version": "24.01.000", "uri": "../flows/98daf38a-7a79-46d3-9a37-2b7bd0955810.xml"}, "exchange direction": "OUTPUT", "other": {"anies": [{"value": "0", "module": "A1-A3"}, {"name": "referenceToUnitGroupDataSet", "value": {"shortDescription": [{"value": "MJ", "lang": "en"}], "type": "unit group data set", "refObjectId": "93a60a57-a3c8-11da-a746-0800200c9a66", "version": "03.00.000", "uri": "../unitgroups/93a60a57-a3c8-11da-a746-0800200c9a66.xml"}}, {"value": "0", "module": "C2"}, {"value": "12.9903454724284", "module": "C3"}, {"value": "0", "module": "D"}]}, "resolvedFlowVersion": "38.00.000", "flowProperties": [], "typeOfFlow": "Other flow", "classification": {"classHierarchy": "Quantities / Environmental quantities / EPD EN 15804 / LCI indicators", "name": "GaBiCategories"}}]}, "LCIAResults": {"LCIAResult": [{"referenceToLCIAMethodDataSet": {"shortDescription": [{"value": "Climate change", "lang": "en"}, {"value": "Globales Erwärmungspotenzial - total (GWP-total)", "lang": "de"}], "type": "LCIA method data set", "refObjectId": "a7ea142a-9749-11ed-a8fc-0242ac120002", "version": "24.01.000", "uri": "../lciamethods/a7ea142a-9749-11ed-a8fc-0242ac120002.xml"}, "other": {"anies": [{"value": "4.30685708675401", "module": "A1-A3"}, {"value": "0.00340594400973465", "module": "C2"}, {"value": "2.87438641134717", "module": "C3"}, {"value": "-1.5148494424377", "module": "D"}, {"name": "referenceToUnitGroupDataSet", "value": {"shortDescription": [{"value": "kg CO2 eq.", "lang": "en"}], "type": "unit group data set", "refObjectId": "1ebf3012-d0db-4de2-aefd-ef30cedb0be1", "version": "25.00.000", "uri": "../unitgroups/1ebf3012-d0db-4de2-aefd-ef30cedb0be1.xml"}}]}}, {"referenceToLCIAMethodDataSet": {"shortDescription": [{"value": "Climate change-Fossil", "lang": "en"}, {"value": "Globales Erwärmungspotenzial - fossil (GWP-fossil)", "lang": "de"}], "type": "LCIA method data set", "refObjectId": "a7ea19c0-9749-11ed-a8fc-0242ac120002", "version": "24.01.000", "uri": "../lciamethods/a7ea19c0-9749-11ed-a8fc-0242ac120002.xml"}, "other": {"anies": [{"value": "4.28078297985106", "module": "A1-A3"}, {"value": "0.00332467008188178", "module": "C2"}, {"value": "2.87413333277309", "module": "C3"}, {"value": "-1.50382444569835", "module": "D"}, {"name": "referenceToUnitGroupDataSet", "value": {"shortDescription": [{"value": "kg CO2 eq.", "lang": "en"}], "type": "unit group data set", "refObjectId": "1ebf3012-d0db-4de2-aefd-ef30cedb0be1", "version": "25.00.000", "uri": "../unitgroups/1ebf3012-d0db-4de2-aefd-ef30cedb0be1.xml"}}]}}, {"referenceToLCIAMethodDataSet": {"shortDescription": [{"value": "Climate change-Biogenic", "lang": "en"}, {"value": "Globales Erwärmungspotenzial - biogen (GWP-biogenic)", "lang": "de"}], "type": "LCIA method data set", "refObjectId": "a7ea186c-9749-11ed-a8fc-0242ac120002", "version": "24.01.000", "uri": "../lciamethods/a7ea186c-9749-11ed-a8fc-0242ac120002.xml"}, "other": {"anies": [{"value": "0.0254350246484095", "module": "A1-A3"}, {"value": "1.72994093894545E-5", "module": "C2"}, {"value": "0.000209764171067292", "module": "C3"}, {"value": "-0.0108392986213768", "module": "D"}, {"name": "referenceToUnitGroupDataSet", "value": {"shortDescription": [{"value": "kg CO2 eq.", "lang": "en"}], "type": "unit group data set", "refObjectId": "1ebf3012-d0db-4de2-aefd-ef30cedb0be1", "version": "25.00.000", "uri": "../unitgroups/1ebf3012-d0db-4de2-aefd-ef30cedb0be1.xml"}}]}}, {"referenceToLCIAMethodDataSet": {"shortDescription": [{"value": "Climate change-Land use and land use change", "lang": "en"}, {"value": "Globales Erwärmungspotenzial - luluc (GWP-luluc)", "lang": "de"}], "type": "LCIA method data set", "refObjectId": "a7ea1ae2-9749-11ed-a8fc-0242ac120002", "version": "24.01.000", "uri": "../lciamethods/a7ea1ae2-9749-11ed-a8fc-0242ac120002.xml"}, "other": {"anies": [{"value": "0.000639082254540107", "module": "A1-A3"}, {"value": "6.39745184634203E-5", "module": "C2"}, {"value": "4.33144030090379E-5", "module": "C3"}, {"value": "-0.000185698117972886", "module": "D"}, {"name": "referenceToUnitGroupDataSet", "value": {"shortDescription": [{"value": "kg CO2 eq.", "lang": "en"}], "type": "unit group data set", "refObjectId": "1ebf3012-d0db-4de2-aefd-ef30cedb0be1", "version": "25.00.000", "uri": "../unitgroups/1ebf3012-d0db-4de2-aefd-ef30cedb0be1.xml"}}]}}, {"referenceToLCIAMethodDataSet": {"shortDescription": [{"value": "Depletion potenzial of the stratospheric ozone layer (ODP)", "lang": "en"}, {"value": "Abbaupotenzial der stratosphärischen Ozonschicht (ODP)", "lang": "de"}], "type": "LCIA method data set", "refObjectId": "b5c629d6-def3-11e6-bf01-fe55135034f3", "version": "24.01.000", "uri": "../lciamethods/b5c629d6-def3-11e6-bf01-fe55135034f3.xml"}, "other": {"anies": [{"value": "2.21443270658857E-11", "module": "A1-A3"}, {"value": "1.05030066685908E-15", "module": "C2"}, {"value": "4.14430827417939E-13", "module": "C3"}, {"value": "-2.30160391851483E-11", "module": "D"}, {"name": "referenceToUnitGroupDataSet", "value": {"shortDescription": [{"value": "kg CFC-11 eq.", "lang": "en"}], "type": "unit group data set", "refObjectId": "d9e957c9-7309-4474-bf3a-7777df6c4e5b", "version": "25.00.000", "uri": "../unitgroups/d9e957c9-7309-4474-bf3a-7777df6c4e5b.xml"}}]}}, {"referenceToLCIAMethodDataSet": {"shortDescription": [{"value": "Acidifcation potential, Accumulated Exceedance (AP)", "lang": "en"}, {"value": "Versauerungspotenzial, kumulierte Überschreitung (AP)", "lang": "de"}], "type": "LCIA method data set", "refObjectId": "b5c611c6-def3-11e6-bf01-fe55135034f3", "version": "24.01.000", "uri": "../lciamethods/b5c611c6-def3-11e6-bf01-fe55135034f3.xml"}, "other": {"anies": [{"value": "0.00458293994802927", "module": "A1-A3"}, {"value": "1.05576421403198E-5", "module": "C2"}, {"value": "0.000391224882284836", "module": "C3"}, {"value": "-0.00150388799933499", "module": "D"}, {"name": "referenceToUnitGroupDataSet", "value": {"shortDescription": [{"value": "Mole of H+ eq.", "lang": "en"}], "type": "unit group data set", "refObjectId": "42e089ac-92bf-4bf2-8ca1-5fc40d18f2ed", "version": "00.01.000", "uri": "../unitgroups/42e089ac-92bf-4bf2-8ca1-5fc40d18f2ed.xml"}}]}}, {"referenceToLCIAMethodDataSet": {"shortDescription": [{"value": "Eutrophication, freshwater", "lang": "en"}, {"value": "Eutrophierungspotenzial - Süßwasser (EP-freshwater)", "lang": "de"}], "type": "LCIA method data set", "refObjectId": "b53ec18f-7377-4ad3-86eb-cc3f4f276b2b", "version": "24.01.000", "uri": "../lciamethods/b53ec18f-7377-4ad3-86eb-cc3f4f276b2b.xml"}, "other": {"anies": [{"value": "6.78445241236885E-6", "module": "A1-A3"}, {"value": "9.05742233605885E-9", "module": "C2"}, {"value": "1.22663805981204E-7", "module": "C3"}, {"value": "-3.73449038887822E-6", "module": "D"}, {"name": "referenceToUnitGroupDataSet", "value": {"shortDescription": [{"value": "kg P eq.", "lang": "en"}], "type": "unit group data set", "refObjectId": "0429039d-a61d-4590-ba67-aa4a20a810a1", "version": "25.00.000", "uri": "../unitgroups/0429039d-a61d-4590-ba67-aa4a20a810a1.xml"}}]}}, {"referenceToLCIAMethodDataSet": {"shortDescription": [{"value": "Eutrophication marine", "lang": "en"}, {"value": "Eutrophierungspotenzial - Salzwasser (EP-marine)", "lang": "de"}], "type": "LCIA method data set", "refObjectId": "b5c619fa-def3-11e6-bf01-fe55135034f3", "version": "24.01.000", "uri": "../lciamethods/b5c619fa-def3-11e6-bf01-fe55135034f3.xml"}, "other": {"anies": [{"value": "0.00145005177594612", "module": "A1-A3"}, {"value": "4.81283173745398E-6", "module": "C2"}, {"value": "8.00736855379271E-5", "module": "C3"}, {"value": "-0.000526090091873062", "module": "D"}, {"name": "referenceToUnitGroupDataSet", "value": {"shortDescription": [{"value": "kg N eq.", "lang": "en"}], "type": "unit group data set", "refObjectId": "d05bb823-ecdf-4686-8c40-bf1d9257859f", "version": "00.00.003", "uri": "../unitgroups/d05bb823-ecdf-4686-8c40-bf1d9257859f.xml"}}]}}, {"referenceToLCIAMethodDataSet": {"shortDescription": [{"value": "Eutrophication, terrestrial", "lang": "en"}, {"value": "Eutrophierungspotenzial - Land (EP-terrestrial)", "lang": "de"}], "type": "LCIA method data set", "refObjectId": "b5c614d2-def3-11e6-bf01-fe55135034f3", "version": "24.01.000", "uri": "../lciamethods/b5c614d2-def3-11e6-bf01-fe55135034f3.xml"}, "other": {"anies": [{"value": "0.015431537327494", "module": "A1-A3"}, {"value": "5.44496916520546E-5", "module": "C2"}, {"value": "0.00184780354355446", "module": "C3"}, {"value": "-0.00559306832754051", "module": "D"}, {"name": "referenceToUnitGroupDataSet", "value": {"shortDescription": [{"value": "Mole of N eq.", "lang": "en"}], "type": "unit group data set", "refObjectId": "71b4d617-0ec9-4d3f-b65e-e438940c2401", "version": "00.00.003", "uri": "../unitgroups/71b4d617-0ec9-4d3f-b65e-e438940c2401.xml"}}]}}, {"referenceToLCIAMethodDataSet": {"shortDescription": [{"value": "Photochemical Ozone Creation Potential  (POCP)", "lang": "en"}, {"value": "Bildungspotenzial für troposphärisches Ozon (POCP)", "lang": "de"}], "type": "LCIA method data set", "refObjectId": "b5c610fe-def3-11e6-bf01-fe55135034f3", "version": "24.01.000", "uri": "../lciamethods/b5c610fe-def3-11e6-bf01-fe55135034f3.xml"}, "other": {"anies": [{"value": "0.00509213172720962", "module": "A1-A3"}, {"value": "9.99907939783911E-6", "module": "C2"}, {"value": "0.000215177973699288", "module": "C3"}, {"value": "-0.00138560306219408", "module": "D"}, {"name": "referenceToUnitGroupDataSet", "value": {"shortDescription": [{"value": "kg NMVOC eq.", "lang": "en"}], "type": "unit group data set", "refObjectId": "d27c25f8-fbc1-44c6-b47b-4adbae4199c6", "version": "00.00.003", "uri": "../unitgroups/d27c25f8-fbc1-44c6-b47b-4adbae4199c6.xml"}}]}}, {"referenceToLCIAMethodDataSet": {"shortDescription": [{"value": "Resource use, minerals and metals", "lang": "en"}, {"value": "Potenzial für die Verknappung abiotischer Ressourcen  nicht fossile Ressourcen (ADPE)", "lang": "de"}], "type": "LCIA method data set", "refObjectId": "b2ad6494-c78d-11e6-9d9d-cec0c932ce01", "version": "24.01.000", "uri": "../lciamethods/b2ad6494-c78d-11e6-9d9d-cec0c932ce01.xml"}, "other": {"anies": [{"value": "6.09022818773466E-7", "module": "A1-A3"}, {"value": "5.6443177325321E-10", "module": "C2"}, {"value": "3.44085771582644E-9", "module": "C3"}, {"value": "-1.41680702123488E-7", "module": "D"}, {"name": "referenceToUnitGroupDataSet", "value": {"shortDescription": [{"value": "kg Sb eq.", "lang": "en"}], "type": "unit group data set", "refObjectId": "54ccd2d9-a32a-4fc2-923d-f2c8c93e89d4", "version": "25.00.000", "uri": "../unitgroups/54ccd2d9-a32a-4fc2-923d-f2c8c93e89d4.xml"}}]}}, {"referenceToLCIAMethodDataSet": {"shortDescription": [{"value": "Resource use, fossils", "lang": "en"}, {"value": "Potenzial für die Verknappung abiotischer Ressourcen  fossile Brennstoffe (ADPF)", "lang": "de"}], "type": "LCIA method data set", "refObjectId": "b2ad6110-c78d-11e6-9d9d-cec0c932ce01", "version": "24.01.000", "uri": "../lciamethods/b2ad6110-c78d-11e6-9d9d-cec0c932ce01.xml"}, "other": {"anies": [{"value": "110.652401520395", "module": "A1-A3"}, {"value": "0.0436710870361919", "module": "C2"}, {"value": "0.524749633047421", "module": "C3"}, {"value": "-21.1646084074767", "module": "D"}, {"name": "referenceToUnitGroupDataSet", "value": {"shortDescription": [{"value": "MJ", "lang": "en"}], "type": "unit group data set", "refObjectId": "93a60a57-a3c8-11da-a746-0800200c9a66", "version": "02.00.000", "uri": "../unitgroups/93a60a57-a3c8-11da-a746-0800200c9a66.xml"}}]}}, {"referenceToLCIAMethodDataSet": {"shortDescription": [{"value": "Water use", "lang": "en"}, {"value": "Wasser-Entzugspotenzial (Benutzer) (WDP)", "lang": "de"}], "type": "LCIA method data set", "refObjectId": "b2ad66ce-c78d-11e6-9d9d-cec0c932ce01", "version": "24.01.000", "uri": "../lciamethods/b2ad66ce-c78d-11e6-9d9d-cec0c932ce01.xml"}, "other": {"anies": [{"value": "0.0772142787445902", "module": "A1-A3"}, {"value": "2.38393471046832E-5", "module": "C2"}, {"value": "0.316522743690759", "module": "C3"}, {"value": "-0.0197442684768947", "module": "D"}, {"name": "referenceToUnitGroupDataSet", "value": {"shortDescription": [{"value": "m³ world equiv.", "lang": "en"}], "type": "unit group data set", "refObjectId": "6ae2df01-888e-46c8-b17d-49fa3869b476", "version": "00.00.003", "uri": "../unitgroups/6ae2df01-888e-46c8-b17d-49fa3869b476.xml"}}]}}]}, "otherAttributes": {"{http://www.indata.network/EPD/2019}epd-version": "1.2"}, "version": "1.1", "locations": "../ILCDLocations.xml"}