{"processInformation": {"dataSetInformation": {"UUID": "4b0f5c51-622e-4af8-81f0-c9f13ea7b6b0", "name": {"baseName": [{"value": "BauderTHERMOPLEX", "lang": "de"}, {"value": "BauderTHERMOPLEX", "lang": "en"}], "functionalUnitFlowProperties": [{"lang": "de"}]}, "classificationInformation": {"classification": [{"class": [{"value": "Kunststoffe", "level": 0, "classId": "6"}, {"value": "Dachbahnen", "level": 1, "classId": "6.3"}, {"value": "TPO-Dachbahnen (FPO)", "level": 2, "classId": "6.3.05"}], "name": "OEKOBAU.DAT"}, {"class": [{"value": "02 Bauprodukte", "level": 0}, {"value": "Abdichtungen", "level": 1}, {"value": "Dach- und Dichtungsbahnsysteme aus Kunststoffen und Elastomeren", "level": 2}], "name": "IBUCategories"}]}, "generalComment": [{"value": "BauderTHERMOPLEX sind Kunststoffdachbahnen auf Basis von flexiblen Polyolefinen (FPO) mit einer Verstärkung aus Synthesefasern. Die Produktpalette besteht aus:\n\nBauderTHERMOPLEX P (15/18/20) \nmittige Verstärkung aus Synthesefasern \n\nDie ausgewiesenen Ergebnisse deklarieren einen Durchschnitt über alle BauderTHERMOPLEX-Produkte. Die Durchschnittsbildung basiert auf den entsprechenden Produktionsmengen (nach produzierter Fläche) für das Kalenderjahr 2020.", "lang": "de"}, {"value": "BauderTHERMOPLEX are plastic roofing membranes based on flexible polyolefins (FPO) with a reinforcement of synthetic fibres. The product range consists of: \n\nBauderTHERMOPLEX P (15/18/20)          Embedded reinforcement [C1] made of synthetic fibres\n\n\nThe reported results declare an average across all BauderTHERMOPLEX products. The averaging is based on the corresponding production quantities (by area produced) for the calendar year 2020.", "lang": "en"}], "other": {"anies": [{"scenario": [{"description": [{"value": "Szenario 0", "lang": "de"}, {"value": "Scenario 0", "lang": "en"}], "name": "S0"}, {"description": [{"value": "100% Recycling", "lang": "de"}, {"value": "100% Recycling", "lang": "en"}], "name": "S1", "default": true}, {"description": [{"value": "100% energetische Verwertung", "lang": "de"}, {"value": "100% Energy Recovery", "lang": "en"}], "name": "S2"}]}]}}, "quantitativeReference": {"referenceToReferenceFlow": [0]}, "time": {"referenceYear": 2022, "dataSetValidUntil": 2027, "other": {"anies": [{"name": "publicationDateOfEPD", "value": 1666224000000}]}}, "geography": {"locationOfOperationSupplyOrProduction": {"location": "DE"}}, "technology": {"technologyDescriptionAndIncludedProcesses": [{"value": "Die Fertigung der FPO Dachbahnen erfolgt in einem einstufigen Verfahren. Die Mischung und Plastifizierung der Rohstoffe auf den Extrudern erfolgt getrennt für Ober- und Unterfolie. Die Verstärkungslage wird zuerst mit der Unterfolie danach mit der Oberfolie beschichtet. Nach Abkühlung und endgültigem Randbeschnitt werden die Produkte konfektioniert. Alle anfallenden Produktionsabfälle werden recycelt und dem Fertigungsprozess direkt wieder zugeführt. Eine permanente Messung der Produktqualität und kontinuierliche Verbesserung der internen Prozesse wird durch den Einsatz des Qualitätsmanagement-systems nach /DIN EN ISO 9001/ gewährleistet. \nDeklarierte Einheit: \nDie deklarierte Einheit ist die Herstellung von 1 m² des nach der Produktionsmenge gewichteten Mittels für die mechanisch oder unter Auflast befestigten, mittels Heißluft abgedichteten BauderTHERMOPLEX Dachbahn-Varianten (15/18/20) inklusive Verpackungsmaterialien.", "lang": "de"}, {"value": "FPO roofing membranes are manufactured in a single-stage process. The mixing and plasticising of the raw materials on the extruders is carried out separately for top and bottom film. The reinforcing layer is first coated with the bottom film, then with the top film. After cooling and final edge trimming, the products are made up. All production waste is treated internally. Recyclable fractions are recycled and directly reintroduced into the production process. Non-recyclable components are disposed of. Permanent measurement of product quality and continuous improvement of internal processes is ensured through the use of the ISO 9001 quality management system. \nDeclared unit: \nThe declared unit is the production of 1 m² of the production quantity weighted average for the mechanically or ballasted, hot air sealed BauderTHERMOPLEX roofing membrane variants (15/18/20) including packaging materials.", "lang": "en"}], "technologicalApplicability": [{"value": "Die FPO Dachbahnen werden einlagig verlegt und an den Nähten heißluftverschweißt. Die Windsogsicherung erfolgt durch mechanische Befestigung oder per Auflast.\n\nDachabdichtung – Einlagige Abdichtung von nicht genutzten und genutzten Dächern in flacher und geneigter Form.  \n\nBauderTHERMOPLEX Dachbahnen werden je nach Anforderung: \n\n·         mechanisch befestigt oder\n\n·         unter Auflast verlegt.", "lang": "de"}, {"value": "The FPO roofing membranes are laid in a single layer and hot-air welded at the seams. The wind suction is secured by mechanical fastening or by ballast.\n\nRoof waterproofing \n\nSingle-ply waterproofing of non-utilized and utilized roofs (e.g., solar roof, green roof) in flat and pitched form.\n\n\nBauderTHERMOPLEX roofing membranes are used according to requirements: \n\n- mechanically fixed or                                 \n\n- ballasted.", "lang": "en"}]}}, "modellingAndValidation": {"LCIMethodAndAllocation": {"typeOfDataSet": "EPD", "referenceToLCAMethodDetails": [{"shortDescription": [{"value": "Dach- und Dichtungsbahnsysteme aus Kunststoffen und Elastomeren.pdf", "lang": "de"}], "type": "source data set", "refObjectId": "c0e4f3ef-33ae-43da-9317-09dfb1db4410"}], "other": {"anies": [{"name": "subType", "value": "average dataset"}]}}, "dataSourcesTreatmentAndRepresentativeness": {"referenceToDataSource": [{"shortDescription": [{"value": "GaBi Database (all versions)", "lang": "de"}], "type": "source data set", "refObjectId": "28d74cc0-db8b-4d7e-bc44-5f6d56ce0c4a"}, {"shortDescription": [{"value": "GaBi Database Edition 2022, CUP 2022.02", "lang": "de"}], "type": "source data set", "refObjectId": "94f442cb-662e-43ea-a792-4b0a35132e93"}], "useAdviceForDataSet": [{"value": "Gültigkeitsbereich: \nDieses Dokument ist gültig für die FPO Dachbahnen: \n\n·          BauderTHERMOPLEX P (15/18/20),  \n\nhergestellt im deutschen BAUDER Produktionswerk Schwepnitz. \nSystemgrenze: \nTyp der EPD: von der Wiege bis zum Werkstor mit Optionen (Module A1–A3, C1–C4 und Modul D).  \n\nDeklariert werden gemäß EN 15804 die Module A1–A5, C1–C4 und D. Folgende Punkte wurden bei der Erstellung der Ökobilanz berücksichtigt: \n\n\nModul A1–A3 \n\nSämtliche Vorketten der verwendeten Rohstoffe und Materialien sowie deren Beschaffungstransporte. Produktionsprozesse inklusive Energie- und Abfallströme (Wiege bis Werkstor). Anfallende Abfälle werden bis zum End-of-Waste-Status berücksichtigt. \n\n\nModul A4–A5 \n\nDie Transporte zur Baustelle und ein durchschnittlicher Installationsaufwand (Heißluftverklebung und anfallende Verschnitte) sowie Befestigungsmaterial. Verwertung des Verpackungsmaterials. \n\n\nModul C1\n Abriss der Dach- und Dichtungsbahn vom Dach. \n\n\nModul C2-1 \n\nTransporte im Rahmen der Recycling-Route. \n\n\nModul C2-2 \n\nTransporte im Rahmen der MVA-Route. \n\n\nModul C3-1 \n\nStoffliche Verwertung (Recycling) des Produkts inklusive Aufbereitungsaufwand. \n\n\nModul C3-2 \n\nEnergetische Verwertung (Verbrennung in einer MVA). \n\n\nModule D-1 und D-2 Ausweis der durch die Abfallbehandlung in den Modulen A5, C3-1 und C3-2 entstandenen Gutschriften.", "lang": "de"}, {"value": "Scope: \nThis document is valid for FPO roofing membranes: \n\n- BauderTHERMOPLEX P (15/18/20),  \n\nmanufactured at the German BAUDER production plant in Schwepnitz. \nSystem boundary: \nType of EPD: from cradle to gate with options (modules A1-A3, C1-C4 and module D).  \n\nThe modules A1-A5, C1-C4 and D are declared in accordance with EN 15804. The following points were taken into account in the preparation of the life cycle assessment: \n\n\nModule A1-A3 \n\nAll upstream chains of the raw materials and materials used as well as their procurement transports. Production processes including energy and waste flows (cradle to factory gate). Waste produced is taken into account up to the end-of-waste status. \n\n\nModule A4-A5 \n\nThe transports to the construction site and an average installation effort (hot air bonding and resulting offcuts) as well as fastening material. Recycling of the packaging material. \n\n\nModule C1\n Tearing off the roofing and waterproofing membrane from the roof. \n\n\nModule C2-1 \n\nTransports as part of the recycling route. \n\n\nModule C2-2 \n\nTransports as part of the energy recovery route. \n\n\nModule C3-1 \n\nMaterial recovery (recycling) of the product, including processing costs. \n\n\nModule C3-2 \n\nEnergy recovery (incineration in a waste incineration plant). \n\n\nModules D-1 and D-2 \n\nReporting of credits generated by waste treatment in modules A5, C3-1 and C3-2.", "lang": "en"}], "other": {"anies": [{"name": "referenceToOriginalEPD", "value": {"shortDescription": {"value": "BauderTHERMOPLEX.pdf", "defaultValue": "BauderTHERMOPLEX.pdf", "lstrings": [{"lang": "de", "value": "BauderTHERMOPLEX.pdf"}]}, "type": "source data set", "uuid": {"uuid": "8ec47e25-b392-4a6f-bb7f-a0d0389b7cff"}, "refObjectId": "8ec47e25-b392-4a6f-bb7f-a0d0389b7cff", "resourceURLs": ["https://oekobaudat.de/OEKOBAU.DAT/resource/sources/8ec47e25-b392-4a6f-bb7f-a0d0389b7cff/BauderTHERMOPLEX_15701.pdf?version=00.02.000"]}}]}}, "validation": {"review": [{"referenceToNameOfReviewerAndInstitution": [{"shortDescription": [{"value": "Institut Bauen und Umwelt e. V.", "lang": "de"}], "type": "contact data set", "refObjectId": "d111dbec-b024-4be5-86c5-752d6eb2cf95", "uri": "../contacts/d111dbec-b024-4be5-86c5-752d6eb2cf95.xml"}], "type": "Accredited third party review"}]}, "complianceDeclarations": {"compliance": [{"referenceToComplianceSystem": {"shortDescription": [{"value": "DIN EN 15804+A2", "lang": "de"}], "type": "source data set", "refObjectId": "c0016b33-8cf7-415c-ac6e-deba0d21440d", "uri": "../sources/c0016b33-8cf7-415c-ac6e-deba0d21440d.xml"}}, {"referenceToComplianceSystem": {"shortDescription": [{"value": "ISO 14025", "lang": "de"}], "type": "source data set", "refObjectId": "4f2eb655-6e44-4874-a95a-e28f5442cd4d", "uri": "../sources/4f2eb655-6e44-4874-a95a-e28f5442cd4d.xml"}}]}}, "administrativeInformation": {"commissionerAndGoal": {"referenceToCommissioner": [{"shortDescription": [{"value": "Paul Bauder GmbH & Co. KG", "lang": "de"}], "type": "contact data set", "refObjectId": "1046a2e0-2955-495d-ac78-f874ecd43f62", "uri": "../contacts/1046a2e0-2955-495d-ac78-f874ecd43f62.xml"}]}, "dataGenerator": {"referenceToPersonOrEntityGeneratingTheDataSet": [{"shortDescription": [{"value": "brands and values GmbH", "lang": "de"}], "type": "contact data set", "refObjectId": "6b539b8a-10e3-4004-8ccc-a79f169aa339", "uri": "../contacts/6b539b8a-10e3-4004-8ccc-a79f169aa339.xml"}]}, "dataEntryBy": {"timeStamp": 1666281665003, "referenceToDataSetFormat": [{"shortDescription": [{"value": "ILCD Format", "lang": "de"}], "type": "source data set", "refObjectId": "a97a0155-0234-4b87-b4ce-a45da52f2a40", "uri": "../sources/a97a0155-0234-4b87-b4ce-a45da52f2a40.xml"}, {"shortDescription": [{"value": "EPD-Datenformaterweiterungen v1.2", "lang": "de"}, {"value": "EPD Data Format Extensions v1.2", "lang": "en"}], "type": "source data set", "refObjectId": "a29449fd-aa2f-4de8-b5d7-4b06b43c6fde", "uri": "../sources/a29449fd-aa2f-4de8-b5d7-4b06b43c6fde.xml"}]}, "publicationAndOwnership": {"dataSetVersion": "00.02.000", "referenceToRegistrationAuthority": {"shortDescription": [{"value": "Institut Bauen und Umwelt e. V.", "lang": "de"}], "type": "contact data set", "refObjectId": "d111dbec-b024-4be5-86c5-752d6eb2cf95", "uri": "../contacts/d111dbec-b024-4be5-86c5-752d6eb2cf95.xml"}, "registrationNumber": "EPD-BAU-20220196-IBC1-DE", "referenceToOwnershipOfDataSet": {"shortDescription": [{"value": "Paul Bauder GmbH & Co. KG", "lang": "de"}], "type": "contact data set", "refObjectId": "1046a2e0-2955-495d-ac78-f874ecd43f62", "uri": "../contacts/1046a2e0-2955-495d-ac78-f874ecd43f62.xml"}, "copyright": true, "licenseType": "Free of charge for all users and uses", "accessRestrictions": [{"value": "None", "lang": "en"}], "other": {"anies": [{"name": "referenceToPublisher", "value": {"shortDescription": [{"value": "Institut Bauen und Umwelt e. V.", "lang": "de"}], "type": "contact data set", "refObjectId": "d111dbec-b024-4be5-86c5-752d6eb2cf95", "uri": "../contacts/d111dbec-b024-4be5-86c5-752d6eb2cf95.xml"}}]}}}, "exchanges": {"exchange": [{"dataSetInternalID": 0, "referenceToFlowDataSet": {"shortDescription": [{"value": "BauderTHERMOPLEX P (15/18/20) inkl. Verpackung (BauderTHERMOPLEX P (15/18/20) inkl. Verpackung)", "lang": "de"}], "type": "flow data set", "refObjectId": "58283a4f-b9dd-36d8-a20e-82b444593113", "uri": "../flows/58283a4f-b9dd-36d8-a20e-82b444593113.xml"}, "meanAmount": 1.0, "referencesToDataSource": {}, "referenceFlow": true, "resolvedFlowVersion": "00.02.000", "resultingflowAmount": 1.0, "flowProperties": [{"name": [{"lang": "en", "value": "Area"}, {"lang": "de", "value": "Fläche"}], "uuid": "93a60a56-a3c8-19da-a746-0800200c9a66", "referenceFlowProperty": true, "meanValue": 1.0, "referenceUnit": "qm", "unitGroupUUID": "c20a03d7-bd90-4569-bc94-66cfd364dfc8"}], "materialProperties": [{"name": "layer thickness", "value": "0.0015", "unit": "m", "unitDescription": "meters"}, {"name": "grammage", "value": "1.94", "unit": "kg/m^2", "unitDescription": "kilograms per square meter"}], "typeOfFlow": "Product flow", "classification": {"classHierarchy": "Kunststoffe / Dachbahnen / TPO-Dachbahnen (FPO)", "name": "OEKOBAU.DAT"}}, {"dataSetInternalID": 1, "referenceToFlowDataSet": {"shortDescription": [{"value": "Erneuerbare Primärenergie als Energieträger (PERE)", "lang": "de"}, {"value": "Renewable primary energy as energy carrier (PERE)", "lang": "en"}], "type": "flow data set", "refObjectId": "20f32be5-0398-4288-9b6d-accddd195317", "uri": "../flows/20f32be5-0398-4288-9b6d-accddd195317.xml"}, "exchange direction": "INPUT", "other": {"anies": [{"name": "referenceToUnitGroupDataSet", "value": {"shortDescription": [{"value": "MJ", "lang": "de"}], "type": "unit group data set", "refObjectId": "93a60a57-a3c8-11da-a746-0800200c9a66", "uri": "../unitgroups/93a60a57-a3c8-11da-a746-0800200c9a66.xml"}}, {"value": "4.77851429843728", "module": "A1-A3"}, {"value": "0.106", "module": "A4"}, {"value": "0.997485701562716", "module": "A5"}, {"value": "0.0539", "module": "C1"}, {"value": "0.0261", "module": "C2", "scenario": "S1"}, {"value": "0.00803", "module": "C2", "scenario": "S2"}, {"value": "3.8", "module": "C3", "scenario": "S1"}, {"value": "0.151", "module": "C3", "scenario": "S2"}, {"value": "0", "module": "C4"}, {"value": "-3.39", "module": "D", "scenario": "S1"}, {"value": "-8.08", "module": "D", "scenario": "S2"}]}, "resolvedFlowVersion": "38.00.000", "flowProperties": [], "typeOfFlow": "Other flow", "classification": {"classHierarchy": "Quantities", "name": "GaBiCategories"}}, {"dataSetInternalID": 2, "referenceToFlowDataSet": {"shortDescription": [{"value": "Erneuerbare Primärenergie zur stofflichen Nutzung (PERM)", "lang": "de"}, {"value": "Renewable primary energy resources as material utilization (PERM)", "lang": "en"}], "type": "flow data set", "refObjectId": "fb3ec0de-548d-4508-aea5-00b73bf6f702", "uri": "../flows/fb3ec0de-548d-4508-aea5-00b73bf6f702.xml"}, "exchange direction": "INPUT", "other": {"anies": [{"name": "referenceToUnitGroupDataSet", "value": {"shortDescription": [{"value": "MJ", "lang": "de"}], "type": "unit group data set", "refObjectId": "93a60a57-a3c8-11da-a746-0800200c9a66", "uri": "../unitgroups/93a60a57-a3c8-11da-a746-0800200c9a66.xml"}}, {"value": "0.671485701562716", "module": "A1-A3"}, {"value": "0", "module": "A4"}, {"value": "-0.671485701562716", "module": "A5"}, {"value": "0", "module": "C1"}, {"value": "0", "module": "C2", "scenario": "S1"}, {"value": "0", "module": "C2", "scenario": "S2"}, {"value": "0", "module": "C3", "scenario": "S1"}, {"value": "0", "module": "C3", "scenario": "S2"}, {"value": "0", "module": "C4"}, {"value": "0", "module": "D", "scenario": "S1"}, {"value": "0", "module": "D", "scenario": "S2"}]}, "resolvedFlowVersion": "38.00.000", "flowProperties": [], "typeOfFlow": "Other flow", "classification": {"classHierarchy": "Quantities", "name": "GaBiCategories"}}, {"dataSetInternalID": 3, "referenceToFlowDataSet": {"shortDescription": [{"value": "Total erneuerbare Primärenergie (PERT)", "lang": "de"}, {"value": "Total use of renewable primary energy resources (PERT)", "lang": "en"}], "type": "flow data set", "refObjectId": "53f97275-fa8a-4cdd-9024-65936002acd0", "uri": "../flows/53f97275-fa8a-4cdd-9024-65936002acd0.xml"}, "exchange direction": "INPUT", "other": {"anies": [{"name": "referenceToUnitGroupDataSet", "value": {"shortDescription": [{"value": "MJ", "lang": "de"}], "type": "unit group data set", "refObjectId": "93a60a57-a3c8-11da-a746-0800200c9a66", "uri": "../unitgroups/93a60a57-a3c8-11da-a746-0800200c9a66.xml"}}, {"value": "5.45", "module": "A1-A3"}, {"value": "0.106", "module": "A4"}, {"value": "0.326", "module": "A5"}, {"value": "0.0539", "module": "C1"}, {"value": "0.0261", "module": "C2", "scenario": "S1"}, {"value": "0.00803", "module": "C2", "scenario": "S2"}, {"value": "3.8", "module": "C3", "scenario": "S1"}, {"value": "0.151", "module": "C3", "scenario": "S2"}, {"value": "0", "module": "C4"}, {"value": "-3.39", "module": "D", "scenario": "S1"}, {"value": "-8.08", "module": "D", "scenario": "S2"}]}, "resolvedFlowVersion": "38.00.000", "flowProperties": [], "typeOfFlow": "Other flow", "classification": {"classHierarchy": "Quantities / Environmental quantities / EPD EN 15804 / LCI indicators", "name": "GaBiCategories"}}, {"dataSetInternalID": 4, "referenceToFlowDataSet": {"shortDescription": [{"value": "Nicht-erneuerbare Primärenergie als Energieträger (PENRE)", "lang": "de"}, {"value": "Non renewable primary energy as energy carrier (PENRE)", "lang": "en"}], "type": "flow data set", "refObjectId": "ac857178-2b45-46ec-892a-a9a4332f0372", "uri": "../flows/ac857178-2b45-46ec-892a-a9a4332f0372.xml"}, "exchange direction": "INPUT", "other": {"anies": [{"name": "referenceToUnitGroupDataSet", "value": {"shortDescription": [{"value": "MJ", "lang": "de"}], "type": "unit group data set", "refObjectId": "93a60a57-a3c8-11da-a746-0800200c9a66", "uri": "../unitgroups/93a60a57-a3c8-11da-a746-0800200c9a66.xml"}}, {"value": "37.4579477333984", "module": "A1-A3"}, {"value": "1.54", "module": "A4"}, {"value": "5.64935161988127", "module": "A5"}, {"value": "0.373", "module": "C1"}, {"value": "0.379", "module": "C2", "scenario": "S1"}, {"value": "0.116", "module": "C2", "scenario": "S2"}, {"value": "57.7427006467203", "module": "C3", "scenario": "S1"}, {"value": "49.4727006467203", "module": "C3", "scenario": "S2"}, {"value": "0", "module": "C4"}, {"value": "-77.7", "module": "D", "scenario": "S1"}, {"value": "-30", "module": "D", "scenario": "S2"}]}, "resolvedFlowVersion": "38.00.000", "flowProperties": [], "typeOfFlow": "Other flow", "classification": {"classHierarchy": "Quantities", "name": "GaBiCategories"}}, {"dataSetInternalID": 5, "referenceToFlowDataSet": {"shortDescription": [{"value": "Nicht-erneuerbare Primärenergie zur stofflichen Nutzung (PENRM)", "lang": "de"}, {"value": "Non renewable primary energy as material utilization (PENRM)", "lang": "en"}], "type": "flow data set", "refObjectId": "1421caa0-679d-4bf4-b282-0eb850ccae27", "uri": "../flows/1421caa0-679d-4bf4-b282-0eb850ccae27.xml"}, "exchange direction": "INPUT", "other": {"anies": [{"name": "referenceToUnitGroupDataSet", "value": {"shortDescription": [{"value": "MJ", "lang": "de"}], "type": "unit group data set", "refObjectId": "93a60a57-a3c8-11da-a746-0800200c9a66", "uri": "../unitgroups/93a60a57-a3c8-11da-a746-0800200c9a66.xml"}}, {"value": "48.3420522666016", "module": "A1-A3"}, {"value": "0", "module": "A4"}, {"value": "-0.419351619881265", "module": "A5"}, {"value": "0", "module": "C1"}, {"value": "0", "module": "C2", "scenario": "S1"}, {"value": "0", "module": "C2", "scenario": "S2"}, {"value": "-47.9227006467203", "module": "C3", "scenario": "S1"}, {"value": "-47.9227006467203", "module": "C3", "scenario": "S2"}, {"value": "0", "module": "C4"}, {"value": "0", "module": "D", "scenario": "S1"}, {"value": "0", "module": "D", "scenario": "S2"}]}, "resolvedFlowVersion": "38.00.000", "flowProperties": [], "typeOfFlow": "Other flow", "classification": {"classHierarchy": "Quantities", "name": "GaBiCategories"}}, {"dataSetInternalID": 6, "referenceToFlowDataSet": {"shortDescription": [{"value": "Total nicht erneuerbare Primärenergie (PENRT)", "lang": "de"}, {"value": "Total use of non renewable primary energy resources (PENRT)", "lang": "en"}], "type": "flow data set", "refObjectId": "06159210-646b-4c8d-8583-da9b3b95a6c1", "uri": "../flows/06159210-646b-4c8d-8583-da9b3b95a6c1.xml"}, "exchange direction": "INPUT", "other": {"anies": [{"name": "referenceToUnitGroupDataSet", "value": {"shortDescription": [{"value": "MJ", "lang": "de"}], "type": "unit group data set", "refObjectId": "93a60a57-a3c8-11da-a746-0800200c9a66", "uri": "../unitgroups/93a60a57-a3c8-11da-a746-0800200c9a66.xml"}}, {"value": "85.8", "module": "A1-A3"}, {"value": "1.54", "module": "A4"}, {"value": "5.23", "module": "A5"}, {"value": "0.373", "module": "C1"}, {"value": "0.379", "module": "C2", "scenario": "S1"}, {"value": "0.116", "module": "C2", "scenario": "S2"}, {"value": "9.82", "module": "C3", "scenario": "S1"}, {"value": "1.55", "module": "C3", "scenario": "S2"}, {"value": "0", "module": "C4"}, {"value": "-77.7", "module": "D", "scenario": "S1"}, {"value": "-30", "module": "D", "scenario": "S2"}]}, "resolvedFlowVersion": "38.00.000", "flowProperties": [], "typeOfFlow": "Other flow", "classification": {"classHierarchy": "Quantities / Environmental quantities / EPD EN 15804 / LCI indicators", "name": "GaBiCategories"}}, {"dataSetInternalID": 7, "referenceToFlowDataSet": {"shortDescription": [{"value": "Einsatz von Sekundärstoffen (SM)", "lang": "de"}, {"value": "Use of secondary material (SM)", "lang": "en"}], "type": "flow data set", "refObjectId": "c6a1f35f-2d09-4f54-8dfb-97e502e1ce92", "uri": "../flows/c6a1f35f-2d09-4f54-8dfb-97e502e1ce92.xml"}, "exchange direction": "INPUT", "other": {"anies": [{"name": "referenceToUnitGroupDataSet", "value": {"shortDescription": [{"value": "kg", "lang": "de"}], "type": "unit group data set", "refObjectId": "ad38d542-3fe9-439d-9b95-2f5f7752acaf", "uri": "../unitgroups/ad38d542-3fe9-439d-9b95-2f5f7752acaf.xml"}}, {"value": "0", "module": "A1-A3"}, {"value": "0", "module": "A4"}, {"value": "0", "module": "A5"}, {"value": "0", "module": "C1"}, {"value": "0", "module": "C2", "scenario": "S1"}, {"value": "0", "module": "C2", "scenario": "S2"}, {"value": "0", "module": "C3", "scenario": "S1"}, {"value": "0", "module": "C3", "scenario": "S2"}, {"value": "0", "module": "C4"}, {"value": "1.11", "module": "D", "scenario": "S1"}, {"value": "0.035", "module": "D", "scenario": "S2"}]}, "resolvedFlowVersion": "38.00.000", "flowProperties": [], "typeOfFlow": "Other flow", "classification": {"classHierarchy": "Quantities / Environmental quantities / EPD EN 15804 / LCI indicators", "name": "GaBiCategories"}}, {"dataSetInternalID": 8, "referenceToFlowDataSet": {"shortDescription": [{"value": "Erneuerbare Sekundärbrennstoffe (RSF)", "lang": "de"}, {"value": "Use of renewable secondary fuels (RSF)", "lang": "en"}], "type": "flow data set", "refObjectId": "64333088-a55f-4aa2-9a31-c10b07816787", "uri": "../flows/64333088-a55f-4aa2-9a31-c10b07816787.xml"}, "exchange direction": "INPUT", "other": {"anies": [{"name": "referenceToUnitGroupDataSet", "value": {"shortDescription": [{"value": "MJ", "lang": "de"}], "type": "unit group data set", "refObjectId": "93a60a57-a3c8-11da-a746-0800200c9a66", "uri": "../unitgroups/93a60a57-a3c8-11da-a746-0800200c9a66.xml"}}, {"value": "0", "module": "A1-A3"}, {"value": "0", "module": "A4"}, {"value": "0", "module": "A5"}, {"value": "0", "module": "C1"}, {"value": "0", "module": "C2", "scenario": "S1"}, {"value": "0", "module": "C2", "scenario": "S2"}, {"value": "0", "module": "C3", "scenario": "S1"}, {"value": "0", "module": "C3", "scenario": "S2"}, {"value": "0", "module": "C4"}, {"value": "0", "module": "D", "scenario": "S1"}, {"value": "0", "module": "D", "scenario": "S2"}]}, "resolvedFlowVersion": "38.00.000", "flowProperties": [], "typeOfFlow": "Other flow", "classification": {"classHierarchy": "Quantities / Environmental quantities / EPD EN 15804 / LCI indicators", "name": "GaBiCategories"}}, {"dataSetInternalID": 9, "referenceToFlowDataSet": {"shortDescription": [{"value": "Nicht erneuerbare Sekundärbrennstoffe (NRSF)", "lang": "de"}, {"value": "Use of non renewable secondary fuels (NRSF)", "lang": "en"}], "type": "flow data set", "refObjectId": "89def144-d39a-4287-b86f-efde453ddcb2", "uri": "../flows/89def144-d39a-4287-b86f-efde453ddcb2.xml"}, "exchange direction": "INPUT", "other": {"anies": [{"name": "referenceToUnitGroupDataSet", "value": {"shortDescription": [{"value": "MJ", "lang": "de"}], "type": "unit group data set", "refObjectId": "93a60a57-a3c8-11da-a746-0800200c9a66", "uri": "../unitgroups/93a60a57-a3c8-11da-a746-0800200c9a66.xml"}}, {"value": "0", "module": "A1-A3"}, {"value": "0", "module": "A4"}, {"value": "0", "module": "A5"}, {"value": "0", "module": "C1"}, {"value": "0", "module": "C2", "scenario": "S1"}, {"value": "0", "module": "C2", "scenario": "S2"}, {"value": "0", "module": "C3", "scenario": "S1"}, {"value": "0", "module": "C3", "scenario": "S2"}, {"value": "0", "module": "C4"}, {"value": "0", "module": "D", "scenario": "S1"}, {"value": "0", "module": "D", "scenario": "S2"}]}, "resolvedFlowVersion": "38.00.000", "flowProperties": [], "typeOfFlow": "Other flow", "classification": {"classHierarchy": "Quantities / Environmental quantities / EPD EN 15804 / LCI indicators", "name": "GaBiCategories"}}, {"dataSetInternalID": 10, "referenceToFlowDataSet": {"shortDescription": [{"value": "Einsatz von Süßwasserressourcen (FW)", "lang": "de"}, {"value": "Use of net fresh water (FW)", "lang": "en"}], "type": "flow data set", "refObjectId": "3cf952c8-f3a4-461d-8c96-96456ca62246", "uri": "../flows/3cf952c8-f3a4-461d-8c96-96456ca62246.xml"}, "exchange direction": "INPUT", "other": {"anies": [{"name": "referenceToUnitGroupDataSet", "value": {"shortDescription": [{"value": "m^3", "lang": "de"}], "type": "unit group data set", "refObjectId": "cd950537-0a98-4044-9ba7-9f9a68d0a504", "uri": "../unitgroups/cd950537-0a98-4044-9ba7-9f9a68d0a504.xml"}}, {"value": "0.0303", "module": "A1-A3"}, {"value": "0.000122", "module": "A4"}, {"value": "0.00124", "module": "A5"}, {"value": "8.16E-05", "module": "C1"}, {"value": "3.02E-05", "module": "C2", "scenario": "S1"}, {"value": "9.27E-06", "module": "C2", "scenario": "S2"}, {"value": "0.00403", "module": "C3", "scenario": "S1"}, {"value": "0.0101", "module": "C3", "scenario": "S2"}, {"value": "0", "module": "C4"}, {"value": "-0.00903", "module": "D", "scenario": "S1"}, {"value": "-0.00801", "module": "D", "scenario": "S2"}]}, "resolvedFlowVersion": "38.00.000", "flowProperties": [], "typeOfFlow": "Other flow", "classification": {"classHierarchy": "Quantities / Environmental quantities / EPD EN 15804 / LCI indicators", "name": "GaBiCategories"}}, {"dataSetInternalID": 11, "referenceToFlowDataSet": {"shortDescription": [{"value": "Gefährlicher Abfall zur Deponie (HWD)", "lang": "de"}, {"value": "Hazardous waste disposed (HWD)", "lang": "en"}], "type": "flow data set", "refObjectId": "430f9e0f-59b2-46a0-8e0d-55e0e84948fc", "uri": "../flows/430f9e0f-59b2-46a0-8e0d-55e0e84948fc.xml"}, "exchange direction": "OUTPUT", "other": {"anies": [{"name": "referenceToUnitGroupDataSet", "value": {"shortDescription": [{"value": "kg", "lang": "de"}], "type": "unit group data set", "refObjectId": "ad38d542-3fe9-439d-9b95-2f5f7752acaf", "uri": "../unitgroups/ad38d542-3fe9-439d-9b95-2f5f7752acaf.xml"}}, {"value": "1.77E-08", "module": "A1-A3"}, {"value": "8.13E-12", "module": "A4"}, {"value": "2.97E-10", "module": "A5"}, {"value": "2.67E-11", "module": "C1"}, {"value": "2E-12", "module": "C2", "scenario": "S1"}, {"value": "6.16E-13", "module": "C2", "scenario": "S2"}, {"value": "1.13E-09", "module": "C3", "scenario": "S1"}, {"value": "4.22E-11", "module": "C3", "scenario": "S2"}, {"value": "0", "module": "C4"}, {"value": "-5.67E-09", "module": "D", "scenario": "S1"}, {"value": "-3.98E-09", "module": "D", "scenario": "S2"}]}, "resolvedFlowVersion": "38.00.000", "flowProperties": [], "typeOfFlow": "Other flow", "classification": {"classHierarchy": "Quantities / Environmental quantities / EPD EN 15804 / LCI indicators", "name": "GaBiCategories"}}, {"dataSetInternalID": 12, "referenceToFlowDataSet": {"shortDescription": [{"value": "Entsorgter nicht gefährlicher Abfall (NHWD)", "lang": "de"}, {"value": "Non hazardous waste disposed (NHWD)", "lang": "en"}], "type": "flow data set", "refObjectId": "b29ef66b-e286-4afa-949f-62f1a7b4d7fa", "uri": "../flows/b29ef66b-e286-4afa-949f-62f1a7b4d7fa.xml"}, "exchange direction": "OUTPUT", "other": {"anies": [{"name": "referenceToUnitGroupDataSet", "value": {"shortDescription": [{"value": "kg", "lang": "de"}], "type": "unit group data set", "refObjectId": "ad38d542-3fe9-439d-9b95-2f5f7752acaf", "uri": "../unitgroups/ad38d542-3fe9-439d-9b95-2f5f7752acaf.xml"}}, {"value": "0.0833", "module": "A1-A3"}, {"value": "0.00025", "module": "A4"}, {"value": "0.0053", "module": "A5"}, {"value": "7.92E-05", "module": "C1"}, {"value": "6.17E-05", "module": "C2", "scenario": "S1"}, {"value": "1.9E-05", "module": "C2", "scenario": "S2"}, {"value": "0.204", "module": "C3", "scenario": "S1"}, {"value": "0.0152", "module": "C3", "scenario": "S2"}, {"value": "0", "module": "C4"}, {"value": "-0.0104", "module": "D", "scenario": "S1"}, {"value": "-0.00645", "module": "D", "scenario": "S2"}]}, "resolvedFlowVersion": "38.00.000", "flowProperties": [], "typeOfFlow": "Other flow", "classification": {"classHierarchy": "Quantities / Environmental quantities / EPD EN 15804 / LCI indicators", "name": "GaBiCategories"}}, {"dataSetInternalID": 13, "referenceToFlowDataSet": {"shortDescription": [{"value": "Entsorgter radioaktiver Abfall (RWD)", "lang": "de"}, {"value": "Radioactive waste disposed (RWD)", "lang": "en"}], "type": "flow data set", "refObjectId": "3449546e-52ad-4b39-b809-9fb77cea8ff6", "uri": "../flows/3449546e-52ad-4b39-b809-9fb77cea8ff6.xml"}, "exchange direction": "OUTPUT", "other": {"anies": [{"name": "referenceToUnitGroupDataSet", "value": {"shortDescription": [{"value": "kg", "lang": "de"}], "type": "unit group data set", "refObjectId": "ad38d542-3fe9-439d-9b95-2f5f7752acaf", "uri": "../unitgroups/ad38d542-3fe9-439d-9b95-2f5f7752acaf.xml"}}, {"value": "0.000698", "module": "A1-A3"}, {"value": "2.85E-06", "module": "A4"}, {"value": "0.000158", "module": "A5"}, {"value": "6.2E-05", "module": "C1"}, {"value": "7.03E-07", "module": "C2", "scenario": "S1"}, {"value": "2.16E-07", "module": "C2", "scenario": "S2"}, {"value": "0.00109", "module": "C3", "scenario": "S1"}, {"value": "0.000101", "module": "C3", "scenario": "S2"}, {"value": "0", "module": "C4"}, {"value": "-0.000634", "module": "D", "scenario": "S1"}, {"value": "-0.00233", "module": "D", "scenario": "S2"}]}, "resolvedFlowVersion": "38.00.000", "flowProperties": [], "typeOfFlow": "Other flow", "classification": {"classHierarchy": "Quantities / Environmental quantities / EPD EN 15804 / LCI indicators", "name": "GaBiCategories"}}, {"dataSetInternalID": 14, "referenceToFlowDataSet": {"shortDescription": [{"value": "Komponenten für die Wiederverwendung (CRU)", "lang": "de"}, {"value": "Components for re-use (CRU)", "lang": "en"}], "type": "flow data set", "refObjectId": "a2b32f97-3fc7-4af2-b209-525bc6426f33", "uri": "../flows/a2b32f97-3fc7-4af2-b209-525bc6426f33.xml"}, "exchange direction": "OUTPUT", "other": {"anies": [{"name": "referenceToUnitGroupDataSet", "value": {"shortDescription": [{"value": "kg", "lang": "de"}], "type": "unit group data set", "refObjectId": "ad38d542-3fe9-439d-9b95-2f5f7752acaf", "uri": "../unitgroups/ad38d542-3fe9-439d-9b95-2f5f7752acaf.xml"}}, {"value": "0", "module": "A1-A3"}, {"value": "0", "module": "A4"}, {"value": "0", "module": "A5"}, {"value": "0", "module": "C1"}, {"value": "0", "module": "C2", "scenario": "S1"}, {"value": "0", "module": "C2", "scenario": "S2"}, {"value": "0", "module": "C3", "scenario": "S1"}, {"value": "0", "module": "C3", "scenario": "S2"}, {"value": "0", "module": "C4"}, {"value": "0", "module": "D", "scenario": "S1"}, {"value": "0", "module": "D", "scenario": "S2"}]}, "resolvedFlowVersion": "38.00.000", "flowProperties": [], "typeOfFlow": "Other flow", "classification": {"classHierarchy": "Quantities / Environmental quantities / EPD EN 15804 / LCI indicators", "name": "GaBiCategories"}}, {"dataSetInternalID": 15, "referenceToFlowDataSet": {"shortDescription": [{"value": "Stoffe zum Recycling (MFR)", "lang": "de"}, {"value": "Materials for recycling (MFR)", "lang": "en"}], "type": "flow data set", "refObjectId": "d7fe48a5-4103-49c8-9aae-b0b5dfdbd6ae", "uri": "../flows/d7fe48a5-4103-49c8-9aae-b0b5dfdbd6ae.xml"}, "exchange direction": "OUTPUT", "other": {"anies": [{"name": "referenceToUnitGroupDataSet", "value": {"shortDescription": [{"value": "kg", "lang": "de"}], "type": "unit group data set", "refObjectId": "ad38d542-3fe9-439d-9b95-2f5f7752acaf", "uri": "../unitgroups/ad38d542-3fe9-439d-9b95-2f5f7752acaf.xml"}}, {"value": "0", "module": "A1-A3"}, {"value": "0", "module": "A4"}, {"value": "0", "module": "A5"}, {"value": "0", "module": "C1"}, {"value": "0", "module": "C2", "scenario": "S1"}, {"value": "0", "module": "C2", "scenario": "S2"}, {"value": "1.94", "module": "C3", "scenario": "S1"}, {"value": "0.035", "module": "C3", "scenario": "S2"}, {"value": "0", "module": "C4"}, {"value": "0", "module": "D", "scenario": "S1"}, {"value": "0", "module": "D", "scenario": "S2"}]}, "resolvedFlowVersion": "38.00.000", "flowProperties": [], "typeOfFlow": "Other flow", "classification": {"classHierarchy": "Quantities / Environmental quantities / EPD EN 15804 / LCI indicators", "name": "GaBiCategories"}}, {"dataSetInternalID": 16, "referenceToFlowDataSet": {"shortDescription": [{"value": "Stoffe für die Energierückgewinnung (MER)", "lang": "de"}, {"value": "Materials for energy recovery (MER)", "lang": "en"}], "type": "flow data set", "refObjectId": "59a9181c-3aaf-46ee-8b13-2b3723b6e447", "uri": "../flows/59a9181c-3aaf-46ee-8b13-2b3723b6e447.xml"}, "exchange direction": "OUTPUT", "other": {"anies": [{"name": "referenceToUnitGroupDataSet", "value": {"shortDescription": [{"value": "kg", "lang": "de"}], "type": "unit group data set", "refObjectId": "ad38d542-3fe9-439d-9b95-2f5f7752acaf", "uri": "../unitgroups/ad38d542-3fe9-439d-9b95-2f5f7752acaf.xml"}}, {"value": "0", "module": "A1-A3"}, {"value": "0", "module": "A4"}, {"value": "0", "module": "A5"}, {"value": "0", "module": "C1"}, {"value": "0", "module": "C2", "scenario": "S1"}, {"value": "0", "module": "C2", "scenario": "S2"}, {"value": "0", "module": "C3", "scenario": "S1"}, {"value": "0", "module": "C3", "scenario": "S2"}, {"value": "0", "module": "C4"}, {"value": "0", "module": "D", "scenario": "S1"}, {"value": "0", "module": "D", "scenario": "S2"}]}, "resolvedFlowVersion": "38.00.000", "flowProperties": [], "typeOfFlow": "Other flow", "classification": {"classHierarchy": "Quantities / Environmental quantities / EPD EN 15804 / LCI indicators", "name": "GaBiCategories"}}, {"dataSetInternalID": 17, "referenceToFlowDataSet": {"shortDescription": [{"value": "Exportierte elektrische Energie (EEE)", "lang": "de"}, {"value": "Exported electrical energy (EEE)", "lang": "en"}], "type": "flow data set", "refObjectId": "4da0c987-2b76-40d6-9e9e-82a017aaaf29", "uri": "../flows/4da0c987-2b76-40d6-9e9e-82a017aaaf29.xml"}, "exchange direction": "OUTPUT", "other": {"anies": [{"name": "referenceToUnitGroupDataSet", "value": {"shortDescription": [{"value": "MJ", "lang": "de"}], "type": "unit group data set", "refObjectId": "93a60a57-a3c8-11da-a746-0800200c9a66", "uri": "../unitgroups/93a60a57-a3c8-11da-a746-0800200c9a66.xml"}}, {"value": "0", "module": "A1-A3"}, {"value": "0", "module": "A4"}, {"value": "0.157", "module": "A5"}, {"value": "0", "module": "C1"}, {"value": "0", "module": "C2", "scenario": "S1"}, {"value": "0", "module": "C2", "scenario": "S2"}, {"value": "0", "module": "C3", "scenario": "S1"}, {"value": "7.99", "module": "C3", "scenario": "S2"}, {"value": "0", "module": "C4"}, {"value": "0", "module": "D", "scenario": "S1"}, {"value": "0", "module": "D", "scenario": "S2"}]}, "resolvedFlowVersion": "38.00.000", "flowProperties": [], "typeOfFlow": "Other flow", "classification": {"classHierarchy": "Quantities / Environmental quantities / EPD EN 15804 / LCI indicators", "name": "GaBiCategories"}}, {"dataSetInternalID": 18, "referenceToFlowDataSet": {"shortDescription": [{"value": "Exportierte thermische Energie (EET)", "lang": "de"}, {"value": "Exported thermal energy (EET)", "lang": "en"}], "type": "flow data set", "refObjectId": "98daf38a-7a79-46d3-9a37-2b7bd0955810", "uri": "../flows/98daf38a-7a79-46d3-9a37-2b7bd0955810.xml"}, "exchange direction": "OUTPUT", "other": {"anies": [{"name": "referenceToUnitGroupDataSet", "value": {"shortDescription": [{"value": "MJ", "lang": "de"}], "type": "unit group data set", "refObjectId": "93a60a57-a3c8-11da-a746-0800200c9a66", "uri": "../unitgroups/93a60a57-a3c8-11da-a746-0800200c9a66.xml"}}, {"value": "0", "module": "A1-A3"}, {"value": "0", "module": "A4"}, {"value": "0.279", "module": "A5"}, {"value": "0", "module": "C1"}, {"value": "0", "module": "C2", "scenario": "S1"}, {"value": "0", "module": "C2", "scenario": "S2"}, {"value": "0", "module": "C3", "scenario": "S1"}, {"value": "14.2", "module": "C3", "scenario": "S2"}, {"value": "0", "module": "C4"}, {"value": "0", "module": "D", "scenario": "S1"}, {"value": "0", "module": "D", "scenario": "S2"}]}, "resolvedFlowVersion": "38.00.000", "flowProperties": [], "typeOfFlow": "Other flow", "classification": {"classHierarchy": "Quantities / Environmental quantities / EPD EN 15804 / LCI indicators", "name": "GaBiCategories"}}]}, "LCIAResults": {"LCIAResult": [{"referenceToLCIAMethodDataSet": {"shortDescription": [{"value": "Globales Erwärmungspotenzial total (GWP-total)", "lang": "de"}, {"value": "Global Warming Potential total (GWP-total)", "lang": "en"}], "type": "LCIA method data set", "refObjectId": "6a37f984-a4b3-458a-a20a-64418c145fa2", "uri": "../lciamethods/6a37f984-a4b3-458a-a20a-64418c145fa2.xml"}, "other": {"anies": [{"name": "referenceToUnitGroupDataSet", "value": {"shortDescription": [{"value": "kg CO_(2)-Äq.", "lang": "de"}], "type": "unit group data set", "refObjectId": "1ebf3012-d0db-4de2-aefd-ef30cedb0be1", "uri": "../unitgroups/1ebf3012-d0db-4de2-aefd-ef30cedb0be1.xml"}}, {"value": "3.2", "module": "A1-A3"}, {"value": "0.116", "module": "A4"}, {"value": "0.398", "module": "A5"}, {"value": "0.0176", "module": "C1"}, {"value": "0.0289", "module": "C2", "scenario": "S1"}, {"value": "0.00886", "module": "C2", "scenario": "S2"}, {"value": "0.726", "module": "C3", "scenario": "S1"}, {"value": "3.88", "module": "C3", "scenario": "S2"}, {"value": "0", "module": "C4"}, {"value": "-2.2", "module": "D", "scenario": "S1"}, {"value": "-1.79", "module": "D", "scenario": "S2"}]}}, {"referenceToLCIAMethodDataSet": {"shortDescription": [{"value": "Globales Erwärmungspotenzial fossil (GWP-fossil)", "lang": "de"}, {"value": "Global Warming Potential fossil fuels (GWP-fossil)", "lang": "en"}], "type": "LCIA method data set", "refObjectId": "5f635281-343e-44fb-83df-1971b155e6b6", "uri": "../lciamethods/5f635281-343e-44fb-83df-1971b155e6b6.xml"}, "other": {"anies": [{"name": "referenceToUnitGroupDataSet", "value": {"shortDescription": [{"value": "kg CO_(2)-Äq.", "lang": "de"}], "type": "unit group data set", "refObjectId": "1ebf3012-d0db-4de2-aefd-ef30cedb0be1", "uri": "../unitgroups/1ebf3012-d0db-4de2-aefd-ef30cedb0be1.xml"}}, {"value": "3.22", "module": "A1-A3"}, {"value": "0.115", "module": "A4"}, {"value": "0.373", "module": "A5"}, {"value": "0.0176", "module": "C1"}, {"value": "0.0287", "module": "C2", "scenario": "S1"}, {"value": "0.0088", "module": "C2", "scenario": "S2"}, {"value": "0.726", "module": "C3", "scenario": "S1"}, {"value": "3.88", "module": "C3", "scenario": "S2"}, {"value": "0", "module": "C4"}, {"value": "-2.2", "module": "D", "scenario": "S1"}, {"value": "-1.79", "module": "D", "scenario": "S2"}]}}, {"referenceToLCIAMethodDataSet": {"shortDescription": [{"value": "Globales Erwärmungspotenzial biogen (GWP-biogenic)", "lang": "de"}, {"value": "Global Warming Potential biogenic (GWP-biogenic)", "lang": "en"}], "type": "LCIA method data set", "refObjectId": "2356e1ab-0185-4db5-86e5-16de51c7485c", "uri": "../lciamethods/2356e1ab-0185-4db5-86e5-16de51c7485c.xml"}, "other": {"anies": [{"name": "referenceToUnitGroupDataSet", "value": {"shortDescription": [{"value": "kg CO_(2)-Äq.", "lang": "de"}], "type": "unit group data set", "refObjectId": "1ebf3012-d0db-4de2-aefd-ef30cedb0be1", "uri": "../unitgroups/1ebf3012-d0db-4de2-aefd-ef30cedb0be1.xml"}}, {"value": "-0.0252", "module": "A1-A3"}, {"value": "0", "module": "A4"}, {"value": "0.0252", "module": "A5"}, {"value": "0", "module": "C1"}, {"value": "0", "module": "C2", "scenario": "S1"}, {"value": "0", "module": "C2", "scenario": "S2"}, {"value": "0", "module": "C3", "scenario": "S1"}, {"value": "0", "module": "C3", "scenario": "S2"}, {"value": "0", "module": "C4"}, {"value": "0", "module": "D", "scenario": "S1"}, {"value": "0", "module": "D", "scenario": "S2"}]}}, {"referenceToLCIAMethodDataSet": {"shortDescription": [{"value": "Globales Erwärmungspotenzial luluc (GWP-luluc)", "lang": "de"}, {"value": "Global Warming Potential luluc (GWP-luluc)", "lang": "en"}], "type": "LCIA method data set", "refObjectId": "4331bbdb-978a-490d-8707-eeb047f01a55", "uri": "../lciamethods/4331bbdb-978a-490d-8707-eeb047f01a55.xml"}, "other": {"anies": [{"name": "referenceToUnitGroupDataSet", "value": {"shortDescription": [{"value": "kg CO_(2)-Äq.", "lang": "de"}], "type": "unit group data set", "refObjectId": "1ebf3012-d0db-4de2-aefd-ef30cedb0be1", "uri": "../unitgroups/1ebf3012-d0db-4de2-aefd-ef30cedb0be1.xml"}}, {"value": "0.000919", "module": "A1-A3"}, {"value": "0.000785", "module": "A4"}, {"value": "1.81E-05", "module": "A5"}, {"value": "1.14E-06", "module": "C1"}, {"value": "0.000194", "module": "C2", "scenario": "S1"}, {"value": "5.95E-05", "module": "C2", "scenario": "S2"}, {"value": "9.34E-05", "module": "C3", "scenario": "S1"}, {"value": "4.05E-06", "module": "C3", "scenario": "S2"}, {"value": "0", "module": "C4"}, {"value": "-0.000275", "module": "D", "scenario": "S1"}, {"value": "-0.000192", "module": "D", "scenario": "S2"}]}}, {"referenceToLCIAMethodDataSet": {"shortDescription": [{"value": "Abbau Potential der stratosphärischen Ozonschicht (ODP)", "lang": "de"}, {"value": "Depletion potential of the stratospheric ozone layer (ODP)", "lang": "en"}], "type": "LCIA method data set", "refObjectId": "b5c629d6-def3-11e6-bf01-fe55135034f3", "uri": "../lciamethods/b5c629d6-def3-11e6-bf01-fe55135034f3.xml"}, "other": {"anies": [{"name": "referenceToUnitGroupDataSet", "value": {"shortDescription": [{"value": "kg CFC11-Äq.", "lang": "de"}], "type": "unit group data set", "refObjectId": "d9e957c9-7309-4474-bf3a-7777df6c4e5b", "uri": "../unitgroups/d9e957c9-7309-4474-bf3a-7777df6c4e5b.xml"}}, {"value": "6.41E-10", "module": "A1-A3"}, {"value": "1.14E-14", "module": "A4"}, {"value": "1.9E-10", "module": "A5"}, {"value": "1.74E-13", "module": "C1"}, {"value": "2.82E-15", "module": "C2", "scenario": "S1"}, {"value": "8.67E-16", "module": "C2", "scenario": "S2"}, {"value": "5.53E-12", "module": "C3", "scenario": "S1"}, {"value": "4.5E-09", "module": "C3", "scenario": "S2"}, {"value": "0", "module": "C4"}, {"value": "-6.46E-12", "module": "D", "scenario": "S1"}, {"value": "-1.18E-11", "module": "D", "scenario": "S2"}]}}, {"referenceToLCIAMethodDataSet": {"shortDescription": [{"value": "Versauerungspotenzial von Boden und Wasser (AP)", "lang": "de"}, {"value": "Acidification potential of land and water (AP)", "lang": "en"}], "type": "LCIA method data set", "refObjectId": "b5c611c6-def3-11e6-bf01-fe55135034f3", "uri": "../lciamethods/b5c611c6-def3-11e6-bf01-fe55135034f3.xml"}, "other": {"anies": [{"name": "referenceToUnitGroupDataSet", "value": {"shortDescription": [{"value": "mol H^(+)-Äq.", "lang": "de"}], "type": "unit group data set", "refObjectId": "42e089ac-92bf-4bf2-8ca1-5fc40d18f2ed", "uri": "../unitgroups/42e089ac-92bf-4bf2-8ca1-5fc40d18f2ed.xml"}}, {"value": "0.00517", "module": "A1-A3"}, {"value": "0.00067", "module": "A4"}, {"value": "0.000744", "module": "A5"}, {"value": "2.58E-05", "module": "C1"}, {"value": "9.23E-05", "module": "C2", "scenario": "S1"}, {"value": "2.84E-05", "module": "C2", "scenario": "S2"}, {"value": "0.00101", "module": "C3", "scenario": "S1"}, {"value": "0.000836", "module": "C3", "scenario": "S2"}, {"value": "0", "module": "C4"}, {"value": "-0.00356", "module": "D", "scenario": "S1"}, {"value": "-0.00241", "module": "D", "scenario": "S2"}]}}, {"referenceToLCIAMethodDataSet": {"shortDescription": [{"value": "Eutrophierungspotenzial Süßwasser (EP-freshwater)", "lang": "de"}, {"value": "Eutrophication potential aquatic freshwater (EP-freshwater)", "lang": "en"}], "type": "LCIA method data set", "refObjectId": "b53ec18f-7377-4ad3-86eb-cc3f4f276b2b", "uri": "../lciamethods/b53ec18f-7377-4ad3-86eb-cc3f4f276b2b.xml"}, "other": {"anies": [{"name": "referenceToUnitGroupDataSet", "value": {"shortDescription": [{"value": "kg PO_(4)-Äq.", "lang": "de"}], "type": "unit group data set", "refObjectId": "0429039d-a61d-4590-ba67-aa4a20a810a1", "uri": "../unitgroups/0429039d-a61d-4590-ba67-aa4a20a810a1.xml"}}, {"value": "1.05E-05", "module": "A1-A3"}, {"value": "4.16E-07", "module": "A4"}, {"value": "4.26E-07", "module": "A5"}, {"value": "7.89E-09", "module": "C1"}, {"value": "1.03E-07", "module": "C2", "scenario": "S1"}, {"value": "3.15E-08", "module": "C2", "scenario": "S2"}, {"value": "7.04E-06", "module": "C3", "scenario": "S1"}, {"value": "4.91E-08", "module": "C3", "scenario": "S2"}, {"value": "0", "module": "C4"}, {"value": "-2.73E-06", "module": "D", "scenario": "S1"}, {"value": "-2.4E-06", "module": "D", "scenario": "S2"}]}}, {"referenceToLCIAMethodDataSet": {"shortDescription": [{"value": "Eutrophierungspotenzial Salzwasser (EP-marine)", "lang": "de"}, {"value": "Eutrophication potential aquatic marine (EP-marine)", "lang": "en"}], "type": "LCIA method data set", "refObjectId": "b5c619fa-def3-11e6-bf01-fe55135034f3", "uri": "../lciamethods/b5c619fa-def3-11e6-bf01-fe55135034f3.xml"}, "other": {"anies": [{"name": "referenceToUnitGroupDataSet", "value": {"shortDescription": [{"value": "kg N-Äq.", "lang": "de"}], "type": "unit group data set", "refObjectId": "d05bb823-ecdf-4686-8c40-bf1d9257859f", "uri": "../unitgroups/d05bb823-ecdf-4686-8c40-bf1d9257859f.xml"}}, {"value": "0.00139", "module": "A1-A3"}, {"value": "0.000326", "module": "A4"}, {"value": "0.000178", "module": "A5"}, {"value": "7.06E-06", "module": "C1"}, {"value": "4.19E-05", "module": "C2", "scenario": "S1"}, {"value": "1.29E-05", "module": "C2", "scenario": "S2"}, {"value": "0.000267", "module": "C3", "scenario": "S1"}, {"value": "0.000181", "module": "C3", "scenario": "S2"}, {"value": "0", "module": "C4"}, {"value": "-0.000974", "module": "D", "scenario": "S1"}, {"value": "-0.000641", "module": "D", "scenario": "S2"}]}}, {"referenceToLCIAMethodDataSet": {"shortDescription": [{"value": "Eutrophierungspotenzial Land (EP-terrestrial)", "lang": "de"}, {"value": "Eutrophication potential terrestrial (EP-terrestrial)", "lang": "en"}], "type": "LCIA method data set", "refObjectId": "b5c614d2-def3-11e6-bf01-fe55135034f3", "uri": "../lciamethods/b5c614d2-def3-11e6-bf01-fe55135034f3.xml"}, "other": {"anies": [{"name": "referenceToUnitGroupDataSet", "value": {"shortDescription": [{"value": "mol N-Äq.", "lang": "de"}], "type": "unit group data set", "refObjectId": "71b4d617-0ec9-4d3f-b65e-e438940c2401", "uri": "../unitgroups/71b4d617-0ec9-4d3f-b65e-e438940c2401.xml"}}, {"value": "0.0153", "module": "A1-A3"}, {"value": "0.00361", "module": "A4"}, {"value": "0.00175", "module": "A5"}, {"value": "7.54E-05", "module": "C1"}, {"value": "0.00047", "module": "C2", "scenario": "S1"}, {"value": "0.000145", "module": "C2", "scenario": "S2"}, {"value": "0.00273", "module": "C3", "scenario": "S1"}, {"value": "0.00286", "module": "C3", "scenario": "S2"}, {"value": "0", "module": "C4"}, {"value": "-0.0103", "module": "D", "scenario": "S1"}, {"value": "-0.00682", "module": "D", "scenario": "S2"}]}}, {"referenceToLCIAMethodDataSet": {"shortDescription": [{"value": "Bildungspotential für troposphärisches Ozon (POCP)", "lang": "de"}, {"value": "Formation potential of tropospheric ozone photochemical oxidants (POCP)", "lang": "en"}], "type": "LCIA method data set", "refObjectId": "b5c610fe-def3-11e6-bf01-fe55135034f3", "uri": "../lciamethods/b5c610fe-def3-11e6-bf01-fe55135034f3.xml"}, "other": {"anies": [{"name": "referenceToUnitGroupDataSet", "value": {"shortDescription": [{"value": "kg NMVOC-Äq.", "lang": "de"}], "type": "unit group data set", "refObjectId": "d27c25f8-fbc1-44c6-b47b-4adbae4199c6", "uri": "../unitgroups/d27c25f8-fbc1-44c6-b47b-4adbae4199c6.xml"}}, {"value": "0.00472", "module": "A1-A3"}, {"value": "0.00063", "module": "A4"}, {"value": "0.000561", "module": "A5"}, {"value": "1.99E-05", "module": "C1"}, {"value": "8.29E-05", "module": "C2", "scenario": "S1"}, {"value": "2.55E-05", "module": "C2", "scenario": "S2"}, {"value": "0.000699", "module": "C3", "scenario": "S1"}, {"value": "0.000521", "module": "C3", "scenario": "S2"}, {"value": "0", "module": "C4"}, {"value": "-0.0035", "module": "D", "scenario": "S1"}, {"value": "-0.00182", "module": "D", "scenario": "S2"}]}}, {"referenceToLCIAMethodDataSet": {"shortDescription": [{"value": "Potenzial für den abiotischen Abbau nicht fossiler Ressourcen (ADPE)", "lang": "de"}, {"value": "Abiotic depletion potential for non fossil resources (ADPE)", "lang": "en"}], "type": "LCIA method data set", "refObjectId": "b2ad6494-c78d-11e6-9d9d-cec0c932ce01", "uri": "../lciamethods/b2ad6494-c78d-11e6-9d9d-cec0c932ce01.xml"}, "other": {"anies": [{"name": "referenceToUnitGroupDataSet", "value": {"shortDescription": [{"value": "kg Sb-Äq.", "lang": "de"}], "type": "unit group data set", "refObjectId": "54ccd2d9-a32a-4fc2-923d-f2c8c93e89d4", "uri": "../unitgroups/54ccd2d9-a32a-4fc2-923d-f2c8c93e89d4.xml"}}, {"value": "4.92E-07", "module": "A1-A3"}, {"value": "1.17E-08", "module": "A4"}, {"value": "6.95E-06", "module": "A5"}, {"value": "2.09E-09", "module": "C1"}, {"value": "2.9E-09", "module": "C2", "scenario": "S1"}, {"value": "8.9E-10", "module": "C2", "scenario": "S2"}, {"value": "1.12E-07", "module": "C3", "scenario": "S1"}, {"value": "3.99E-09", "module": "C3", "scenario": "S2"}, {"value": "0", "module": "C4"}, {"value": "-5.2E-07", "module": "D", "scenario": "S1"}, {"value": "-4.13E-07", "module": "D", "scenario": "S2"}]}}, {"referenceToLCIAMethodDataSet": {"shortDescription": [{"value": "Potenzial für den abiotischen Abbau fossiler Brennstoffe (ADPF)", "lang": "de"}, {"value": "Abiotic depletion potential for fossil resources (ADPF)", "lang": "en"}], "type": "LCIA method data set", "refObjectId": "b2ad6110-c78d-11e6-9d9d-cec0c932ce01", "uri": "../lciamethods/b2ad6110-c78d-11e6-9d9d-cec0c932ce01.xml"}, "other": {"anies": [{"name": "referenceToUnitGroupDataSet", "value": {"shortDescription": [{"value": "MJ", "lang": "de"}], "type": "unit group data set", "refObjectId": "93a60a57-a3c8-11da-a746-0800200c9a66", "uri": "../unitgroups/93a60a57-a3c8-11da-a746-0800200c9a66.xml"}}, {"value": "85.7", "module": "A1-A3"}, {"value": "1.53", "module": "A4"}, {"value": "5.22", "module": "A5"}, {"value": "0.373", "module": "C1"}, {"value": "0.377", "module": "C2", "scenario": "S1"}, {"value": "0.116", "module": "C2", "scenario": "S2"}, {"value": "9.82", "module": "C3", "scenario": "S1"}, {"value": "1.55", "module": "C3", "scenario": "S2"}, {"value": "0", "module": "C4"}, {"value": "-77.6", "module": "D", "scenario": "S1"}, {"value": "-30", "module": "D", "scenario": "S2"}]}}, {"referenceToLCIAMethodDataSet": {"shortDescription": [{"value": "Wassernutzung (WDP)", "lang": "de"}, {"value": "Water use (WDP)", "lang": "en"}], "type": "LCIA method data set", "refObjectId": "b2ad66ce-c78d-11e6-9d9d-cec0c932ce01", "uri": "../lciamethods/b2ad66ce-c78d-11e6-9d9d-cec0c932ce01.xml"}, "other": {"anies": [{"name": "referenceToUnitGroupDataSet", "value": {"shortDescription": [{"value": "m^(3) Welt-Äq. entzogen", "lang": "de"}], "type": "unit group data set", "refObjectId": "6ae2df01-888e-46c8-b17d-49fa3869b476", "uri": "../unitgroups/6ae2df01-888e-46c8-b17d-49fa3869b476.xml"}}, {"value": "1.02", "module": "A1-A3"}, {"value": "0.0013", "module": "A4"}, {"value": "0.0422", "module": "A5"}, {"value": "0.00131", "module": "C1"}, {"value": "0.000321", "module": "C2", "scenario": "S1"}, {"value": "9.85E-05", "module": "C2", "scenario": "S2"}, {"value": "0.103", "module": "C3", "scenario": "S1"}, {"value": "0.432", "module": "C3", "scenario": "S2"}, {"value": "0", "module": "C4"}, {"value": "-0.163", "module": "D", "scenario": "S1"}, {"value": "-0.194", "module": "D", "scenario": "S2"}]}}, {"referenceToLCIAMethodDataSet": {"shortDescription": [{"value": "Auftreten von Krankheiten aufgrund von Feinstaubemissionen (PM)", "lang": "de"}, {"value": "Incidence of disease due to PM emissions (PM)", "lang": "en"}], "type": "LCIA method data set", "refObjectId": "b5c602c6-def3-11e6-bf01-fe55135034f3", "uri": "../lciamethods/b5c602c6-def3-11e6-bf01-fe55135034f3.xml"}, "other": {"anies": [{"name": "referenceToUnitGroupDataSet", "value": {"shortDescription": [{"value": "Krankheitsfälle", "lang": "de"}], "type": "unit group data set", "refObjectId": "3883559b-648f-4afc-8ba2-0bd24f3affa3", "uri": "../unitgroups/3883559b-648f-4afc-8ba2-0bd24f3affa3.xml"}}, {"module": "A1-A3"}, {"module": "A4"}, {"module": "A5"}, {"module": "C1"}, {"module": "C2", "scenario": "S1"}, {"module": "C2", "scenario": "S2"}, {"module": "C3", "scenario": "S1"}, {"module": "C3", "scenario": "S2"}, {"module": "C4"}, {"module": "D", "scenario": "S1"}, {"module": "D", "scenario": "S2"}]}}, {"referenceToLCIAMethodDataSet": {"shortDescription": [{"value": "Wirkung durch Exposition des Menschen mit U235 (IR)", "lang": "de"}, {"value": "Human exposure efficiency relative to U235 (IR)", "lang": "en"}], "type": "LCIA method data set", "refObjectId": "b5c632be-def3-11e6-bf01-fe55135034f3", "uri": "../lciamethods/b5c632be-def3-11e6-bf01-fe55135034f3.xml"}, "other": {"anies": [{"name": "referenceToUnitGroupDataSet", "value": {"shortDescription": [{"value": "kBq U235-Äq.", "lang": "de"}], "type": "unit group data set", "refObjectId": "456b05bf-1415-44a9-9993-02452f554c09", "uri": "../unitgroups/456b05bf-1415-44a9-9993-02452f554c09.xml"}}, {"module": "A1-A3"}, {"module": "A4"}, {"module": "A5"}, {"module": "C1"}, {"module": "C2", "scenario": "S1"}, {"module": "C2", "scenario": "S2"}, {"module": "C3", "scenario": "S1"}, {"module": "C3", "scenario": "S2"}, {"module": "C4"}, {"module": "D", "scenario": "S1"}, {"module": "D", "scenario": "S2"}]}}, {"referenceToLCIAMethodDataSet": {"shortDescription": [{"value": "Toxizitätsvergleichseinheit für Ökosysteme (ETP-fw)", "lang": "de"}, {"value": "Comparative toxic unit for ecosystems (ETP-fw)", "lang": "en"}], "type": "LCIA method data set", "refObjectId": "ee1082d1-b0f7-43ca-a1f0-21e2a4a74511", "uri": "../lciamethods/ee1082d1-b0f7-43ca-a1f0-21e2a4a74511.xml"}, "other": {"anies": [{"name": "referenceToUnitGroupDataSet", "value": {"shortDescription": [{"value": "CTUe", "lang": "de"}], "type": "unit group data set", "refObjectId": "aa959ded-f1eb-4efb-9c5c-2d60be36b3e6", "uri": "../unitgroups/aa959ded-f1eb-4efb-9c5c-2d60be36b3e6.xml"}}, {"module": "A1-A3"}, {"module": "A4"}, {"module": "A5"}, {"module": "C1"}, {"module": "C2", "scenario": "S1"}, {"module": "C2", "scenario": "S2"}, {"module": "C3", "scenario": "S1"}, {"module": "C3", "scenario": "S2"}, {"module": "C4"}, {"module": "D", "scenario": "S1"}, {"module": "D", "scenario": "S2"}]}}, {"referenceToLCIAMethodDataSet": {"shortDescription": [{"value": "Toxizitätsvergleichseinheit für Menschen (krebserregend) (HTP-c)", "lang": "de"}, {"value": "Comparative toxic unit for humans (carcinogenic) (HTP-c)", "lang": "en"}], "type": "LCIA method data set", "refObjectId": "2299222a-bbd8-474f-9d4f-4dd1f18aea7c", "uri": "../lciamethods/2299222a-bbd8-474f-9d4f-4dd1f18aea7c.xml"}, "other": {"anies": [{"name": "referenceToUnitGroupDataSet", "value": {"shortDescription": [{"value": "CTUh", "lang": "de"}], "type": "unit group data set", "refObjectId": "d4c9523e-2d7e-49fd-8469-998f547d3a70", "uri": "../unitgroups/d4c9523e-2d7e-49fd-8469-998f547d3a70.xml"}}, {"module": "A1-A3"}, {"module": "A4"}, {"module": "A5"}, {"module": "C1"}, {"module": "C2", "scenario": "S1"}, {"module": "C2", "scenario": "S2"}, {"module": "C3", "scenario": "S1"}, {"module": "C3", "scenario": "S2"}, {"module": "C4"}, {"module": "D", "scenario": "S1"}, {"module": "D", "scenario": "S2"}]}}, {"referenceToLCIAMethodDataSet": {"shortDescription": [{"value": "Toxizitätsvergleichseinheit für Menschen (nicht krebserregend) (HTP-nc)", "lang": "de"}, {"value": "Comparative toxic unit for humans (noncarcinogenic) (HTP-nc)", "lang": "en"}], "type": "LCIA method data set", "refObjectId": "3af763a5-b7a1-48c9-9cee-1f223481fcef", "uri": "../lciamethods/3af763a5-b7a1-48c9-9cee-1f223481fcef.xml"}, "other": {"anies": [{"name": "referenceToUnitGroupDataSet", "value": {"shortDescription": [{"value": "CTUh", "lang": "de"}], "type": "unit group data set", "refObjectId": "d4c9523e-2d7e-49fd-8469-998f547d3a70", "uri": "../unitgroups/d4c9523e-2d7e-49fd-8469-998f547d3a70.xml"}}, {"module": "A1-A3"}, {"module": "A4"}, {"module": "A5"}, {"module": "C1"}, {"module": "C2", "scenario": "S1"}, {"module": "C2", "scenario": "S2"}, {"module": "C3", "scenario": "S1"}, {"module": "C3", "scenario": "S2"}, {"module": "C4"}, {"module": "D", "scenario": "S1"}, {"module": "D", "scenario": "S2"}]}}, {"referenceToLCIAMethodDataSet": {"shortDescription": [{"value": "Bodenqualitätsindex (SQP)", "lang": "de"}, {"value": "Soil quality index (SQP)", "lang": "en"}], "type": "LCIA method data set", "refObjectId": "b2ad6890-c78d-11e6-9d9d-cec0c932ce01", "uri": "../lciamethods/b2ad6890-c78d-11e6-9d9d-cec0c932ce01.xml"}, "other": {"anies": [{"name": "referenceToUnitGroupDataSet", "value": {"shortDescription": [{"value": "SQP", "lang": "de"}], "type": "unit group data set", "refObjectId": "f130951c-e67f-4f7f-8dd4-665de3974e18", "uri": "../unitgroups/f130951c-e67f-4f7f-8dd4-665de3974e18.xml"}}, {"module": "A1-A3"}, {"module": "A4"}, {"module": "A5"}, {"module": "C1"}, {"module": "C2", "scenario": "S1"}, {"module": "C2", "scenario": "S2"}, {"module": "C3", "scenario": "S1"}, {"module": "C3", "scenario": "S2"}, {"module": "C4"}, {"module": "D", "scenario": "S1"}, {"module": "D", "scenario": "S2"}]}}]}, "otherAttributes": {"{http://www.indata.network/EPD/2019}epd-version": "1.2"}, "version": "1.1", "locations": "../ILCDLocations.xml"}