{"processInformation": {"dataSetInformation": {"UUID": "566fdbef-3dac-4ed1-bfd3-4337b4bfd5a4", "name": {"baseName": [{"value": "REYSIPUR® Compact High-Pressure Laminate", "lang": "en"}, {"value": "REYSIPUR® Kompakt-Hochdrucklaminat", "lang": "de"}], "functionalUnitFlowProperties": [{"lang": "en"}]}, "classificationInformation": {"classification": [{"class": [{"value": "Holz", "level": 0, "classId": "3"}, {"value": "Holzwerkstoffe", "level": 1, "classId": "3.2"}, {"value": "Wood-Plastic-Composites", "level": 2, "classId": "3.2.09"}], "name": "OEKOBAU.DAT"}, {"class": [{"value": "02 Building products", "level": 0}, {"value": "Interior facilitys", "level": 1}, {"value": "Decorative board for interior use", "level": 2}], "name": "IBUCategories"}]}, "generalComment": [{"value": "REYSIPUR® Compact High-Pressure Laminate panels are 2 decorative-sided high-pressure laminates (HPL) in accordance with EN 438 and ISO 4586. \n\nREYSIPUR® Compact panels consist of layers of fibrous cellulose (usually paper) impregnated with thermosetting synthetic resins that cure under heat and high pressure. \nThe decorative layers are decorative paper impregnated with melamine resin and the core is composed of layers of kraft paper impregnated with phenolic resin.\nThe process, a simultaneous application of heat and high specific pressure enables the flow and subsequent curing of the thermosetting synthetic resins to obtain a homogeneous and non-porous material (bulk density ≥ 1.35 g/cm) with the required surface. \nEssentially, REYSIPUR® Compact consists of more than 60 % paper and the remaining approximately 30 to 40 % consists of phenol-formaldehyde resin for the core layers and melamine-formaldehyde resin for the decorative top layer. \n\nREYSIPUR® Compact panels are characterised by their aesthetic qualities, strength, durability and functional performance. The sheets are available in a wide variety of colours, patterns and surface finishes. They are resistant to wear, impact, scratching, moisture, heat, staining and light resistance and possess good hygienic and anti-static properties. COMPACT are easy to clean and maintain.\nThick REYSIPUR® Compact panels are self-supporting for up to 8mm. They can be used for furniture or wall panelling. For wall panelling, they are typically glued or mechanically fixed on substructure (wood or metallic).\n\nREYSIPUR® Compact boards are available in a variety of dimensions, thicknesses (2 mm to 20 mm) and surface finishes. If flame-retardant Compact is required, the black laminate core can be provided with a halogen-free additive. \nPOLYREY surfaces have antibacterial properties thanks to a treatment based on an active biocidal substance : silver borophosphate glass. This contributes to surface hygiene. \n\nThe declared product is Compact thickness of 8 mm and an average grammage of 10.8 kg/m.", "lang": "en"}, {"value": "REYSIPUR® Compact Hochdrucklaminatplatten sind 2 dekorative Hochdrucklaminate (HPL) gemäß EN 438 und ISO 4586. \n\nREYSIPUR® Compact-Platten bestehen aus Schichten von Faserzellulose (in der Regel Papier), die mit duroplastischen Kunstharzen imprägniert sind, die unter Hitze und hohem Druck aushärten. \nDie Dekorschichten sind mit Melaminharz imprägniertes Dekorpapier und der Kern besteht aus Schichten von mit Phenolharz imprägniertem Kraftpapier. Das Verfahren, eine gleichzeitige Anwendung von Hitze und hohem spezifischem Druck, ermöglicht das Fließen und anschließende Aushärten der duroplastischen Kunstharze, um ein homogenes und porenfreies Material (Schüttdichte ≥ 1,35 g/cm³) mit der gewünschten Oberfläche zu erhalten. \nIm Wesentlichen besteht REYSIPUR® Compact aus mehr als 60 % Papier und die restlichen ca. 30 bis 40 % aus Phenol-Formaldehydharz für die Kernschichten und Melamin-Formaldehydharz für die dekorative Deckschicht. \n\nREYSIPUR® Compact-Platten zeichnen sich durch ihre ästhetischen Qualitäten, ihre Festigkeit, Haltbarkeit und funktionelle Leistung aus. Die Platten sind in einer großen Auswahl an Farben, Mustern und Oberflächenausführungen erhältlich. Sie sind verschleißfest, stoßfest, kratzfest, feuchtigkeits-, hitze-, flecken- und lichtbeständig und verfügen über gute hygienische und antistatische Eigenschaften. COMPACT sind leicht zu reinigen und zu pflegen. Die dicken REYSIPUR® Compact-Platten sind bis zu 8 mm selbsttragend. Sie können für Möbel oder Wandverkleidungen verwendet werden. Für Wandverkleidungen werden sie in der Regel auf eine Unterkonstruktion (Holz oder Metall) geklebt oder mechanisch befestigt. REYSIPUR® Compact-Platten sind in einer Vielzahl von Abmessungen, Stärken (2 mm bis 20 mm) und Oberflächenausführungen erhältlich. Wenn Sie eine schwer entflammbare Compact-Platte benötigen, kann der schwarze Schichtstoffkern mit einem halogenfreien Zusatz versehen werden. \nDie Oberflächen von POLYREY haben antibakterielle Eigenschaften dank einer Behandlung auf der Basis eines bioziden Wirkstoffs: Silberborophosphatglas. Dies trägt zur Oberflächenhygiene bei. \n\nDas deklarierte Produkt hat eine kompakte Dicke von 8 mm und ein durchschnittliches Gewicht von 10,8 kg/m².", "lang": "de"}]}, "quantitativeReference": {"referenceToReferenceFlow": [0]}, "time": {"referenceYear": 2025, "dataSetValidUntil": 2030, "other": {"anies": [{"name": "publicationDateOfEPD", "value": 1742947200000}]}}, "geography": {"locationOfOperationSupplyOrProduction": {"location": "RER"}}, "technology": {"technologyDescriptionAndIncludedProcesses": [{"value": "The manufacturing process involves resin production, resin treating and drying, collation and assembly, pressing and cutting to size: Resin: Two resins are used in the production of REYSIPUR® Compact : phenol-formaldehyde and melamine-formaldehyde resins for treating of the core papers and for treatment of the overlay and decorative papers.The phenolic and melamine resins are produced on Polyrey's site. Resin Treating and Drying: During the treating and drying step, papers are mechanically fed through a resin bath and then heated in an oven to cure the resin. Collation and Assembly: During collation (of the core sheets) and assembly (of the decorative and overlay sheets) sheets of treated and untreated paper are stacked both manually and mechanically. This step is in preparation of the pressing stage. Pressing: During pressing, the collated core and assembled decorative/overlay sheets are brought together to be pressed into the laminate product using stainless steel plates and high temperature and pressure. The output of the pressing process is the laminate product. Untreated kraft paper is used as a protective layer and a thermal barrier between the textured metal plates and the heated press platens. Triming : During this finishing step, panels are trimed lenght and width to their standard size.Then panels are shipped in their standard size to the fabricator. \nTechnical data: \nREYSIPUR® Compact are tested and assessed in accordance with EN 438-2. The product requirements can be found in Part 4 of the EN 438 series of standards. Further information can be found in the product data sheet available on our website http://www.polyrey.com. \nDeclared unit: \nThe declared unit is 1 m2 of REYSIPUR® Compact product with 8 mm thickness for the compact with a density of at least 1350 kg/m.", "lang": "en"}, {"value": "Der Herstellungsprozess umfasst die Produktion von Harz, die Behandlung und Trocknung des Harzes, die Zusammenstellung und Montage, das Pressen und den Zuschnitt:\n\nHarz: Für die Herstellung von REYSIPUR® Compact werden zwei Harze verwendet: Phenol-Formaldehyd- und Melamin-Formaldehyd-Harze für die Behandlung der Kernpapiere und für die Behandlung der Overlay- und Dekorpapiere. Die Phenol- und Melaminharze werden am Standort von Polyrey hergestellt.\n\nBehandlung und Trocknung des Harzes: Während des Behandlungs- und Trocknungsschritts werden die Papiere mechanisch durch ein Harzbad geführt und anschließend in einem Ofen erhitzt, um das Harz zu härten.\n\nZusammentragen und Zusammenfügen: Während des Zusammentragens (der Kernblätter) und des Zusammenfügens (der Dekor- und Overlayblätter) werden Blätter aus behandeltem und unbehandeltem Papier sowohl manuell als auch maschinell gestapelt. Dieser Schritt dient der Vorbereitung des Pressvorgangs.\nPressen: Beim Pressen werden die zusammengetragenen Kern- und zusammengesetzten Dekor-/Overlay-Bögen zusammengeführt, um mit Hilfe von Edelstahlplatten unter hoher Temperatur und hohem Druck zu einem Laminatprodukt gepresst zu werden. Das Ergebnis des Pressvorgangs ist das Laminatprodukt. Unbehandeltes Kraftpapier wird als Schutzschicht und thermische Barriere zwischen den strukturierten Metallplatten und den beheizten Pressplatten verwendet.\n\nZuschneiden: Bei diesem Arbeitsschritt werden die Platten in Länge und Breite auf ihre Standardgröße zugeschnitten und in ihrer Standardgröße an den Verarbeiter geliefert. \nTechnische Daten: \nREYSIPUR® Compact wird gemäß EN 438-2 getestet und bewertet. Die Produktanforderungen finden Sie in Teil 4 der Normenreihe EN 438. Weitere Informationen finden Sie im Produktdatenblatt, das Sie auf unserer Website http://www.polyrey.com finden. \nDeklarierte Einheit: \nDie deklarierte Einheit ist 1 m2 des Produkts REYSIPUR® Compact mit einer Dicke von 8 mm für den Verdichter mit einer Dichte von mindestens 1350 kg/m³.", "lang": "de"}], "technologicalApplicability": [{"value": "REYSIPUR® Compact High-Pressure Laminate according to EN 438-4 is a surface material with excellent properties such as durability, cleanability, resistance to wear and to impact, combined with a wide range of technical and creative possibilities.\nREYSIPUR® Compact is self supporting starting from 8 mm.\n\nREYSIPUR® Compact can be used for private and -residential housing, hospitals and laboratories, public buildings, railway stations, airport terminals/infrastructure, transportation, hotels, education, retail and commercial buildings, sport & recreation centres and industrial buildings.\nThe performance properties of REYSIPUR® Compact make it ideal for use in heavy-duty environments, including damp environments : wall cladding, railing infill panels, furniture, tables, desks, column cladding and lab equipment, cubicles, ceilings, window sills, worktops, countertops, etc.", "lang": "en"}, {"value": "REYSIPUR® Compact Hochdrucklaminat nach EN 438-4 ist ein Oberflächenmaterial mit hervorragenden Eigenschaften wie Langlebigkeit, Reinigungsfähigkeit, Verschleiß- und Stoßfestigkeit, kombiniert mit einer breiten Palette an technischen und gestalterischen Möglichkeiten. REYSIPUR® Compact ist ab 8 mm selbsttragend.\n\nREYSIPUR® Compact kann für Privat- und Wohngebäude, Krankenhäuser und Labors, öffentliche Gebäude, Bahnhöfe, Flughafenterminals/Infrastruktur, Transportwesen, Hotels, Bildungseinrichtungen, Einzelhandels- und Gewerbegebäude, Sport- und Freizeitzentren und Industriegebäude verwendet werden. Die Leistungseigenschaften von REYSIPUR® Compact machen es ideal für den Einsatz in stark beanspruchten Umgebungen, einschließlich feuchter Umgebungen: Wandverkleidungen, Geländerfüllungen, Möbel, Tische, Schreibtische, Säulenverkleidungen und Laborgeräte, Kabinen, Decken, Fensterbänke, Arbeitsplatten, Arbeitsflächen usw.", "lang": "de"}]}}, "modellingAndValidation": {"LCIMethodAndAllocation": {"typeOfDataSet": "EPD", "referenceToLCAMethodDetails": [{"shortDescription": [{"value": "Decorative board for interior use.pdf", "lang": "en"}], "type": "source data set", "refObjectId": "b65f8313-00fa-4a53-8d95-799360fae4e8"}], "other": {"anies": [{"name": "subType", "value": "specific dataset"}]}}, "dataSourcesTreatmentAndRepresentativeness": {"referenceToDataSource": [{"shortDescription": [{"value": "GaBi Database (all versions)", "lang": "en"}], "type": "source data set", "refObjectId": "28d74cc0-db8b-4d7e-bc44-5f6d56ce0c4a"}, {"shortDescription": [{"value": "GaBi Database Edition 2022, CUP 2022.01", "lang": "en"}], "type": "source data set", "refObjectId": "86f664e2-7dab-4722-aad7-4c5206a4123b"}], "useAdviceForDataSet": [{"value": "Scope: \nThe declaration relates to thick decorative high-pressure laminates in accordance with EN 438-4 with the product name REYSIPUR® Compact High-Pressure Laminate, which are manufactured at the POLYREY production sites in France (Baneuil and Ussel). The declaration covers the entire range of colours/decors. \nSystem boundary: \nThe life cycle assessment of REYSIPUR® Compact High-Pressure Laminate includes a cradle-to-gate with options and the additional modules are A4, A5 and B1. \nThe following phases of the life cycle are taken into account in the analysis: \n\n• Production of pre-products, extraction of energy carriers, raw material transportation, manufacture of product and packaging materials are declared in modules A1-A3.\nWithin the factory boundaries, the production of phenolic and melamine resin, the impregnation of the papers, the pressing process in the multi-opening presses, the formatting and the packaging are taken into account. The electrical energy used is supplied by the French power grid. Thermal energy is provided as an energy carrier by natural gas, wood chips and production residues.\n\n• The scenario for the transport of the product to the construction site is declared in module A4.\n\n• The treatment of packaging materials at installation, installation auxiliaries, as well as installation losses are declared in module A5\n\n• The use stage includes emissions occurring during the lifetime of the product (B1).\nThe impact associated with maintenance is out of scope (B2). \n\n• The end-of-life scenario is declared in the EPD. They include manual dismantling (C1), transportation to waste processing (C2), and end-of-life scenario 100 % thermal treatment with energy recovery (C3). Credits for electricity and thermal energy, which result from energy recovery in modules A5 and C3, are declared in module D.\n\n• The CO2 incorporation in the product (from the sequestration in the paper material) is considered. The C-balance is closed by considering the biotic CO2 emissions according to the incorporation on the input side.", "lang": "en"}, {"value": "Gültigkeitsbereich: \nDie Deklaration bezieht sich auf dicke dekorative Hochdrucklaminate nach EN 438-4 mit dem Produktnamen REYSIPUR® Kompakt-Hochdrucklaminat, die in den POLYREY-Produktionsstätten in Frankreich (Baneuil und Ussel) hergestellt werden. Die Deklaration deckt die gesamte Palette der Farben/Dekore ab. \nSystemgrenze: \nDie Ökobilanz von REYSIPUR® Kompakt-Hochdrucklaminat umfasst ein Cradle-to-Gate mit Optionen und die zusätzlichen Module sind A4, A5 und B1. \nDie folgenden Phasen des Lebenszyklus werden in der Analyse berücksichtigt: - Die Herstellung von Vorprodukten, die Gewinnung von Energieträgern, der Transport von Rohstoffen, die Herstellung von Produkt- und Verpackungsmaterialien werden in den Modulen A1-A3 angegeben. Innerhalb der Fabrikgrenzen werden die Herstellung von Phenol- und Melaminharz, die Imprägnierung der Papiere, der Pressvorgang in den Mehretagenpressen, die Formatierung und die Verpackung berücksichtigt. Die verwendete elektrische Energie wird aus dem französischen Stromnetz bezogen. Thermische Energie wird als Energieträger durch Erdgas, Holzspäne und Produktionsrückstände bereitgestellt. - Das Szenario für den Transport des Produkts zur Baustelle wird in Modul A4 angegeben. - Die Behandlung von Verpackungsmaterialien bei der Installation, Installationshilfsmittel sowie Installationsverluste werden in Modul A5 angegeben. - Die Nutzungsphase umfasst Emissionen, die während der Lebensdauer des Produkts entstehen (B1). Die Auswirkungen im Zusammenhang mit der Wartung sind nicht berücksichtigt (B2). \n\n- Das End-of-Life-Szenario wird in der EPD angegeben. Dazu gehören die manuelle Demontage (C1), der Transport zur Abfallverarbeitung (C2) und das End-of-Life-Szenario 100 % thermische Behandlung mit Energierückgewinnung (C3). Gutschriften für Strom und thermische Energie, die aus der Energierückgewinnung in den Modulen A5 und C3 resultieren, werden in Modul D angegeben. - Der CO2-Eintrag in das Produkt (aus der Sequestrierung im Papiermaterial) wird berücksichtigt. Die C-Bilanz wird geschlossen, indem die biotischen CO2-Emissionen entsprechend der Einbindung auf der Input-Seite berücksichtigt werden.", "lang": "de"}], "other": {"anies": [{"name": "referenceToOriginalEPD", "value": {"shortDescription": {"value": "REYSIPUR® Compact High-Pressure Laminate.pdf", "defaultValue": "REYSIPUR® Compact High-Pressure Laminate.pdf", "lstrings": [{"lang": "en", "value": "REYSIPUR® Compact High-Pressure Laminate.pdf"}]}, "type": "source data set", "uuid": {"uuid": "470634c5-9321-4309-8558-07aa8787bcf2"}, "refObjectId": "470634c5-9321-4309-8558-07aa8787bcf2", "resourceURLs": ["https://oekobaudat.de/OEKOBAU.DAT/resource/sources/470634c5-9321-4309-8558-07aa8787bcf2/REYSIPUR_Compact_High-Pressure_Laminate_22457.pdf?version=00.01.000"]}}]}}, "validation": {"review": [{"referenceToNameOfReviewerAndInstitution": [{"shortDescription": [{"value": "Institut Bauen und Umwelt e. V.", "lang": "en"}], "type": "contact data set", "refObjectId": "d111dbec-b024-4be5-86c5-752d6eb2cf95", "uri": "../contacts/d111dbec-b024-4be5-86c5-752d6eb2cf95.xml"}], "type": "Accredited third party review"}]}, "complianceDeclarations": {"compliance": [{"referenceToComplianceSystem": {"shortDescription": [{"value": "DIN EN 15804+A2", "lang": "en"}], "type": "source data set", "refObjectId": "c0016b33-8cf7-415c-ac6e-deba0d21440d", "uri": "../sources/c0016b33-8cf7-415c-ac6e-deba0d21440d.xml"}}, {"referenceToComplianceSystem": {"shortDescription": [{"value": "ISO 14025", "lang": "en"}], "type": "source data set", "refObjectId": "4f2eb655-6e44-4874-a95a-e28f5442cd4d", "uri": "../sources/4f2eb655-6e44-4874-a95a-e28f5442cd4d.xml"}}]}}, "administrativeInformation": {"commissionerAndGoal": {"referenceToCommissioner": [{"shortDescription": [{"value": "WILSONART UK", "lang": "en"}], "type": "contact data set", "refObjectId": "212b4800-ed29-4adc-b90f-d61efba0d4aa", "uri": "../contacts/212b4800-ed29-4adc-b90f-d61efba0d4aa.xml"}]}, "dataGenerator": {"referenceToPersonOrEntityGeneratingTheDataSet": [{"shortDescription": [{"value": "WILSONART UK", "lang": "en"}], "type": "contact data set", "refObjectId": "212b4800-ed29-4adc-b90f-d61efba0d4aa", "uri": "../contacts/212b4800-ed29-4adc-b90f-d61efba0d4aa.xml"}]}, "dataEntryBy": {"timeStamp": 1742947200000, "referenceToDataSetFormat": [{"shortDescription": [{"value": "ILCD Format", "lang": "en"}], "type": "source data set", "refObjectId": "a97a0155-0234-4b87-b4ce-a45da52f2a40", "uri": "../sources/a97a0155-0234-4b87-b4ce-a45da52f2a40.xml"}, {"shortDescription": [{"value": "EPD-Datenformaterweiterungen v1.2", "lang": "de"}, {"value": "EPD Data Format Extensions v1.2", "lang": "en"}], "type": "source data set", "refObjectId": "a29449fd-aa2f-4de8-b5d7-4b06b43c6fde", "uri": "../sources/a29449fd-aa2f-4de8-b5d7-4b06b43c6fde.xml"}]}, "publicationAndOwnership": {"dataSetVersion": "00.01.000", "referenceToRegistrationAuthority": {"shortDescription": [{"value": "Institut Bauen und Umwelt e. V.", "lang": "en"}], "type": "contact data set", "refObjectId": "d111dbec-b024-4be5-86c5-752d6eb2cf95", "uri": "../contacts/d111dbec-b024-4be5-86c5-752d6eb2cf95.xml"}, "registrationNumber": "EPD-WIL-20240582-IBA1-EN", "referenceToOwnershipOfDataSet": {"shortDescription": [{"value": "WILSONART UK", "lang": "en"}], "type": "contact data set", "refObjectId": "212b4800-ed29-4adc-b90f-d61efba0d4aa", "uri": "../contacts/212b4800-ed29-4adc-b90f-d61efba0d4aa.xml"}, "copyright": true, "licenseType": "Free of charge for all users and uses", "accessRestrictions": [{"value": "None", "lang": "en"}], "other": {"anies": [{"name": "referenceToPublisher", "value": {"shortDescription": [{"value": "Institut Bauen und Umwelt e. V.", "lang": "en"}], "type": "contact data set", "refObjectId": "d111dbec-b024-4be5-86c5-752d6eb2cf95", "uri": "../contacts/d111dbec-b024-4be5-86c5-752d6eb2cf95.xml"}}]}}}, "exchanges": {"exchange": [{"dataSetInternalID": 0, "referenceToFlowDataSet": {"shortDescription": [{"value": "REYSIPUR® Compact High-Pressure Laminate (Na)", "lang": "en"}], "type": "flow data set", "refObjectId": "3754b0f0-40b5-68d1-4359-92434b570366", "uri": "../flows/3754b0f0-40b5-68d1-4359-92434b570366.xml"}, "meanAmount": 1.0, "referencesToDataSource": {}, "referenceFlow": true, "resolvedFlowVersion": "00.01.000", "resultingflowAmount": 1.0, "flowProperties": [{"name": [{"lang": "de", "value": "Fläche"}, {"lang": "en", "value": "Area"}], "uuid": "93a60a56-a3c8-19da-a746-0800200c9a66", "referenceFlowProperty": true, "meanValue": 1.0, "referenceUnit": "qm", "unitGroupUUID": "c20a03d7-bd90-4569-bc94-66cfd364dfc8"}], "materialProperties": [{"name": "grammage", "value": "10.8", "unit": "kg/m^2", "unitDescription": "kilograms per square meter"}, {"name": "gross density", "value": "1350.0", "unit": "kg/m^3", "unitDescription": "kilograms per cubic metre"}, {"name": "layer thickness", "value": "0.008", "unit": "m", "unitDescription": "meters"}], "typeOfFlow": "Product flow", "classification": {"classHierarchy": "Holz / Holzwerkstoffe / Wood-Plastic-Composites", "name": "OEKOBAU.DAT"}}, {"dataSetInternalID": 1, "referenceToFlowDataSet": {"shortDescription": [{"value": "Renewable primary energy as energy carrier (PERE)", "lang": "en"}, {"value": "Erneuerbare Primärenergie als Energieträger (PERE)", "lang": "de"}], "type": "flow data set", "refObjectId": "20f32be5-0398-4288-9b6d-accddd195317", "uri": "../flows/20f32be5-0398-4288-9b6d-accddd195317.xml"}, "exchange direction": "INPUT", "other": {"anies": [{"name": "referenceToUnitGroupDataSet", "value": {"shortDescription": [{"value": "MJ", "lang": "en"}], "type": "unit group data set", "refObjectId": "93a60a57-a3c8-11da-a746-0800200c9a66", "uri": "../unitgroups/93a60a57-a3c8-11da-a746-0800200c9a66.xml"}}, {"value": "218.804441364751", "module": "A1-A3"}, {"value": "0.879419335066", "module": "A4"}, {"value": "46.5601128328851", "module": "A5"}, {"value": "0", "module": "B1"}, {"value": "0", "module": "C1"}, {"value": "0.0411092626168372", "module": "C2"}, {"value": "104.4160049209", "module": "C3"}, {"value": "0", "module": "C4"}, {"value": "-33.7713028269232", "module": "D"}]}, "resolvedFlowVersion": "38.00.000", "flowProperties": [], "typeOfFlow": "Other flow", "classification": {"classHierarchy": "Quantities", "name": "GaBiCategories"}}, {"dataSetInternalID": 2, "referenceToFlowDataSet": {"shortDescription": [{"value": "Renewable primary energy resources as material utilization (PERM)", "lang": "en"}, {"value": "Erneuerbare Primärenergie zur stofflichen Nutzung (PERM)", "lang": "de"}], "type": "flow data set", "refObjectId": "fb3ec0de-548d-4508-aea5-00b73bf6f702", "uri": "../flows/fb3ec0de-548d-4508-aea5-00b73bf6f702.xml"}, "exchange direction": "INPUT", "other": {"anies": [{"name": "referenceToUnitGroupDataSet", "value": {"shortDescription": [{"value": "MJ", "lang": "en"}], "type": "unit group data set", "refObjectId": "93a60a57-a3c8-11da-a746-0800200c9a66", "uri": "../unitgroups/93a60a57-a3c8-11da-a746-0800200c9a66.xml"}}, {"value": "126.82332", "module": "A1-A3"}, {"value": "0", "module": "A4"}, {"value": "-29.62332", "module": "A5"}, {"value": "0", "module": "B1"}, {"value": "0", "module": "C1"}, {"value": "0", "module": "C2"}, {"value": "-97.2", "module": "C3"}, {"value": "0", "module": "C4"}, {"value": "0", "module": "D"}]}, "resolvedFlowVersion": "38.00.000", "flowProperties": [], "typeOfFlow": "Other flow", "classification": {"classHierarchy": "Quantities", "name": "GaBiCategories"}}, {"dataSetInternalID": 3, "referenceToFlowDataSet": {"shortDescription": [{"value": "Total use of renewable primary energy resources (PERT)", "lang": "en"}, {"value": "Total erneuerbare Primärenergie (PERT)", "lang": "de"}], "type": "flow data set", "refObjectId": "53f97275-fa8a-4cdd-9024-65936002acd0", "uri": "../flows/53f97275-fa8a-4cdd-9024-65936002acd0.xml"}, "exchange direction": "INPUT", "other": {"anies": [{"name": "referenceToUnitGroupDataSet", "value": {"shortDescription": [{"value": "MJ", "lang": "en"}], "type": "unit group data set", "refObjectId": "93a60a57-a3c8-11da-a746-0800200c9a66", "uri": "../unitgroups/93a60a57-a3c8-11da-a746-0800200c9a66.xml"}}, {"value": "345.62776136475", "module": "A1-A3"}, {"value": "0.879419335066", "module": "A4"}, {"value": "16.9367928328851", "module": "A5"}, {"value": "0", "module": "B1"}, {"value": "0", "module": "C1"}, {"value": "0.0411092626168372", "module": "C2"}, {"value": "7.21600492090013", "module": "C3"}, {"value": "0", "module": "C4"}, {"value": "-33.7713028269232", "module": "D"}]}, "resolvedFlowVersion": "38.00.000", "flowProperties": [], "typeOfFlow": "Other flow", "classification": {"classHierarchy": "Quantities / Environmental quantities / EPD EN 15804 / LCI indicators", "name": "GaBiCategories"}}, {"dataSetInternalID": 4, "referenceToFlowDataSet": {"shortDescription": [{"value": "Non renewable primary energy as energy carrier (PENRE)", "lang": "en"}, {"value": "Nicht-erneuerbare Primärenergie als Energieträger (PENRE)", "lang": "de"}], "type": "flow data set", "refObjectId": "ac857178-2b45-46ec-892a-a9a4332f0372", "uri": "../flows/ac857178-2b45-46ec-892a-a9a4332f0372.xml"}, "exchange direction": "INPUT", "other": {"anies": [{"name": "referenceToUnitGroupDataSet", "value": {"shortDescription": [{"value": "MJ", "lang": "en"}], "type": "unit group data set", "refObjectId": "93a60a57-a3c8-11da-a746-0800200c9a66", "uri": "../unitgroups/93a60a57-a3c8-11da-a746-0800200c9a66.xml"}}, {"value": "346.572128224006", "module": "A1-A3"}, {"value": "12.7385537655158", "module": "A4"}, {"value": "17.5795513720557", "module": "A5"}, {"value": "0", "module": "B1"}, {"value": "0", "module": "C1"}, {"value": "0.595475367921027", "module": "C2"}, {"value": "124.718328813443", "module": "C3"}, {"value": "0", "module": "C4"}, {"value": "-61.9916970581241", "module": "D"}]}, "resolvedFlowVersion": "38.00.000", "flowProperties": [], "typeOfFlow": "Other flow", "classification": {"classHierarchy": "Quantities", "name": "GaBiCategories"}}, {"dataSetInternalID": 5, "referenceToFlowDataSet": {"shortDescription": [{"value": "Non renewable primary energy as material utilization (PENRM)", "lang": "en"}, {"value": "Nicht-erneuerbare Primärenergie zur stofflichen Nutzung (PENRM)", "lang": "de"}], "type": "flow data set", "refObjectId": "1421caa0-679d-4bf4-b282-0eb850ccae27", "uri": "../flows/1421caa0-679d-4bf4-b282-0eb850ccae27.xml"}, "exchange direction": "INPUT", "other": {"anies": [{"name": "referenceToUnitGroupDataSet", "value": {"shortDescription": [{"value": "MJ", "lang": "en"}], "type": "unit group data set", "refObjectId": "93a60a57-a3c8-11da-a746-0800200c9a66", "uri": "../unitgroups/93a60a57-a3c8-11da-a746-0800200c9a66.xml"}}, {"value": "105.9605", "module": "A1-A3"}, {"value": "0", "module": "A4"}, {"value": "-8.7605", "module": "A5"}, {"value": "0", "module": "B1"}, {"value": "0", "module": "C1"}, {"value": "0", "module": "C2"}, {"value": "-97.2", "module": "C3"}, {"value": "0", "module": "C4"}, {"value": "0", "module": "D"}]}, "resolvedFlowVersion": "38.00.000", "flowProperties": [], "typeOfFlow": "Other flow", "classification": {"classHierarchy": "Quantities", "name": "GaBiCategories"}}, {"dataSetInternalID": 6, "referenceToFlowDataSet": {"shortDescription": [{"value": "Total use of non renewable primary energy resources (PENRT)", "lang": "en"}, {"value": "Total nicht erneuerbare Primärenergie (PENRT)", "lang": "de"}], "type": "flow data set", "refObjectId": "06159210-646b-4c8d-8583-da9b3b95a6c1", "uri": "../flows/06159210-646b-4c8d-8583-da9b3b95a6c1.xml"}, "exchange direction": "INPUT", "other": {"anies": [{"name": "referenceToUnitGroupDataSet", "value": {"shortDescription": [{"value": "MJ", "lang": "en"}], "type": "unit group data set", "refObjectId": "93a60a57-a3c8-11da-a746-0800200c9a66", "uri": "../unitgroups/93a60a57-a3c8-11da-a746-0800200c9a66.xml"}}, {"value": "452.532628224007", "module": "A1-A3"}, {"value": "12.7385537655159", "module": "A4"}, {"value": "8.81905137205567", "module": "A5"}, {"value": "0", "module": "B1"}, {"value": "0", "module": "C1"}, {"value": "0.595475367921028", "module": "C2"}, {"value": "27.5183288134433", "module": "C3"}, {"value": "0", "module": "C4"}, {"value": "-61.9916970581245", "module": "D"}]}, "resolvedFlowVersion": "38.00.000", "flowProperties": [], "typeOfFlow": "Other flow", "classification": {"classHierarchy": "Quantities / Environmental quantities / EPD EN 15804 / LCI indicators", "name": "GaBiCategories"}}, {"dataSetInternalID": 7, "referenceToFlowDataSet": {"shortDescription": [{"value": "Use of secondary material (SM)", "lang": "en"}, {"value": "Einsatz von Sekundärstoffen (SM)", "lang": "de"}], "type": "flow data set", "refObjectId": "c6a1f35f-2d09-4f54-8dfb-97e502e1ce92", "uri": "../flows/c6a1f35f-2d09-4f54-8dfb-97e502e1ce92.xml"}, "exchange direction": "INPUT", "other": {"anies": [{"name": "referenceToUnitGroupDataSet", "value": {"shortDescription": [{"value": "kg", "lang": "en"}], "type": "unit group data set", "refObjectId": "ad38d542-3fe9-439d-9b95-2f5f7752acaf", "uri": "../unitgroups/ad38d542-3fe9-439d-9b95-2f5f7752acaf.xml"}}, {"value": "0.2088", "module": "A1-A3"}, {"value": "0", "module": "A4"}, {"value": "0", "module": "A5"}, {"value": "0", "module": "B1"}, {"value": "0", "module": "C1"}, {"value": "0", "module": "C2"}, {"value": "0", "module": "C3"}, {"value": "0", "module": "C4"}, {"value": "0", "module": "D"}]}, "resolvedFlowVersion": "38.00.000", "flowProperties": [], "typeOfFlow": "Other flow", "classification": {"classHierarchy": "Quantities / Environmental quantities / EPD EN 15804 / LCI indicators", "name": "GaBiCategories"}}, {"dataSetInternalID": 8, "referenceToFlowDataSet": {"shortDescription": [{"value": "Use of renewable secondary fuels (RSF)", "lang": "en"}, {"value": "Erneuerbare Sekundärbrennstoffe (RSF)", "lang": "de"}], "type": "flow data set", "refObjectId": "64333088-a55f-4aa2-9a31-c10b07816787", "uri": "../flows/64333088-a55f-4aa2-9a31-c10b07816787.xml"}, "exchange direction": "INPUT", "other": {"anies": [{"name": "referenceToUnitGroupDataSet", "value": {"shortDescription": [{"value": "MJ", "lang": "en"}], "type": "unit group data set", "refObjectId": "93a60a57-a3c8-11da-a746-0800200c9a66", "uri": "../unitgroups/93a60a57-a3c8-11da-a746-0800200c9a66.xml"}}, {"value": "0", "module": "A1-A3"}, {"value": "0", "module": "A4"}, {"value": "0", "module": "A5"}, {"value": "0", "module": "B1"}, {"value": "0", "module": "C1"}, {"value": "0", "module": "C2"}, {"value": "0", "module": "C3"}, {"value": "0", "module": "C4"}, {"value": "0", "module": "D"}]}, "resolvedFlowVersion": "38.00.000", "flowProperties": [], "typeOfFlow": "Other flow", "classification": {"classHierarchy": "Quantities / Environmental quantities / EPD EN 15804 / LCI indicators", "name": "GaBiCategories"}}, {"dataSetInternalID": 9, "referenceToFlowDataSet": {"shortDescription": [{"value": "Use of non renewable secondary fuels (NRSF)", "lang": "en"}, {"value": "Nicht erneuerbare Sekundärbrennstoffe (NRSF)", "lang": "de"}], "type": "flow data set", "refObjectId": "89def144-d39a-4287-b86f-efde453ddcb2", "uri": "../flows/89def144-d39a-4287-b86f-efde453ddcb2.xml"}, "exchange direction": "INPUT", "other": {"anies": [{"name": "referenceToUnitGroupDataSet", "value": {"shortDescription": [{"value": "MJ", "lang": "en"}], "type": "unit group data set", "refObjectId": "93a60a57-a3c8-11da-a746-0800200c9a66", "uri": "../unitgroups/93a60a57-a3c8-11da-a746-0800200c9a66.xml"}}, {"value": "0", "module": "A1-A3"}, {"value": "0", "module": "A4"}, {"value": "0", "module": "A5"}, {"value": "0", "module": "B1"}, {"value": "0", "module": "C1"}, {"value": "0", "module": "C2"}, {"value": "0", "module": "C3"}, {"value": "0", "module": "C4"}, {"value": "0", "module": "D"}]}, "resolvedFlowVersion": "38.00.000", "flowProperties": [], "typeOfFlow": "Other flow", "classification": {"classHierarchy": "Quantities / Environmental quantities / EPD EN 15804 / LCI indicators", "name": "GaBiCategories"}}, {"dataSetInternalID": 10, "referenceToFlowDataSet": {"shortDescription": [{"value": "Use of net fresh water (FW)", "lang": "en"}, {"value": "Einsatz von Süßwasserressourcen (FW)", "lang": "de"}], "type": "flow data set", "refObjectId": "3cf952c8-f3a4-461d-8c96-96456ca62246", "uri": "../flows/3cf952c8-f3a4-461d-8c96-96456ca62246.xml"}, "exchange direction": "INPUT", "other": {"anies": [{"name": "referenceToUnitGroupDataSet", "value": {"shortDescription": [{"value": "m^3", "lang": "en"}], "type": "unit group data set", "refObjectId": "cd950537-0a98-4044-9ba7-9f9a68d0a504", "uri": "../unitgroups/cd950537-0a98-4044-9ba7-9f9a68d0a504.xml"}}, {"value": "0.13450868175193", "module": "A1-A3"}, {"value": "0.00101588656912427", "module": "A4"}, {"value": "0.0113458617889533", "module": "A5"}, {"value": "0", "module": "B1"}, {"value": "0", "module": "C1"}, {"value": "4.74885485158376E-05", "module": "C2"}, {"value": "0.0545514028024206", "module": "C3"}, {"value": "0", "module": "C4"}, {"value": "-0.0334620250303219", "module": "D"}]}, "resolvedFlowVersion": "38.00.000", "flowProperties": [], "typeOfFlow": "Other flow", "classification": {"classHierarchy": "Quantities / Environmental quantities / EPD EN 15804 / LCI indicators", "name": "GaBiCategories"}}, {"dataSetInternalID": 11, "referenceToFlowDataSet": {"shortDescription": [{"value": "Hazardous waste disposed (HWD)", "lang": "en"}, {"value": "Gefährlicher Abfall zur Deponie (HWD)", "lang": "de"}], "type": "flow data set", "refObjectId": "430f9e0f-59b2-46a0-8e0d-55e0e84948fc", "uri": "../flows/430f9e0f-59b2-46a0-8e0d-55e0e84948fc.xml"}, "exchange direction": "OUTPUT", "other": {"anies": [{"name": "referenceToUnitGroupDataSet", "value": {"shortDescription": [{"value": "kg", "lang": "en"}], "type": "unit group data set", "refObjectId": "ad38d542-3fe9-439d-9b95-2f5f7752acaf", "uri": "../unitgroups/ad38d542-3fe9-439d-9b95-2f5f7752acaf.xml"}}, {"value": "5.97833010262943E-06", "module": "A1-A3"}, {"value": "6.7402260280346E-11", "module": "A4"}, {"value": "5.86901818561048E-10", "module": "A5"}, {"value": "0", "module": "B1"}, {"value": "0", "module": "C1"}, {"value": "3.15078041651792E-12", "module": "C2"}, {"value": "2.19864859596006E-09", "module": "C3"}, {"value": "0", "module": "C4"}, {"value": "-5.27426301363813E-09", "module": "D"}]}, "resolvedFlowVersion": "38.00.000", "flowProperties": [], "typeOfFlow": "Other flow", "classification": {"classHierarchy": "Quantities / Environmental quantities / EPD EN 15804 / LCI indicators", "name": "GaBiCategories"}}, {"dataSetInternalID": 12, "referenceToFlowDataSet": {"shortDescription": [{"value": "Non hazardous waste disposed (NHWD)", "lang": "en"}, {"value": "Entsorgter nicht gefährlicher Abfall (NHWD)", "lang": "de"}], "type": "flow data set", "refObjectId": "b29ef66b-e286-4afa-949f-62f1a7b4d7fa", "uri": "../flows/b29ef66b-e286-4afa-949f-62f1a7b4d7fa.xml"}, "exchange direction": "OUTPUT", "other": {"anies": [{"name": "referenceToUnitGroupDataSet", "value": {"shortDescription": [{"value": "kg", "lang": "en"}], "type": "unit group data set", "refObjectId": "ad38d542-3fe9-439d-9b95-2f5f7752acaf", "uri": "../unitgroups/ad38d542-3fe9-439d-9b95-2f5f7752acaf.xml"}}, {"value": "0.510702539474113", "module": "A1-A3"}, {"value": "0.00207542740662632", "module": "A4"}, {"value": "0.0842815742271929", "module": "A5"}, {"value": "0", "module": "B1"}, {"value": "0", "module": "C1"}, {"value": "9.70177558067675E-05", "module": "C2"}, {"value": "8.80427872190734", "module": "C3"}, {"value": "0", "module": "C4"}, {"value": "-0.0556541025976376", "module": "D"}]}, "resolvedFlowVersion": "38.00.000", "flowProperties": [], "typeOfFlow": "Other flow", "classification": {"classHierarchy": "Quantities / Environmental quantities / EPD EN 15804 / LCI indicators", "name": "GaBiCategories"}}, {"dataSetInternalID": 13, "referenceToFlowDataSet": {"shortDescription": [{"value": "Radioactive waste disposed (RWD)", "lang": "en"}, {"value": "Entsorgter radioaktiver Abfall (RWD)", "lang": "de"}], "type": "flow data set", "refObjectId": "3449546e-52ad-4b39-b809-9fb77cea8ff6", "uri": "../flows/3449546e-52ad-4b39-b809-9fb77cea8ff6.xml"}, "exchange direction": "OUTPUT", "other": {"anies": [{"name": "referenceToUnitGroupDataSet", "value": {"shortDescription": [{"value": "kg", "lang": "en"}], "type": "unit group data set", "refObjectId": "ad38d542-3fe9-439d-9b95-2f5f7752acaf", "uri": "../unitgroups/ad38d542-3fe9-439d-9b95-2f5f7752acaf.xml"}}, {"value": "0.020240140518721", "module": "A1-A3"}, {"value": "2.36464273832826E-05", "module": "A4"}, {"value": "0.000459863716756572", "module": "A5"}, {"value": "0", "module": "B1"}, {"value": "0", "module": "C1"}, {"value": "1.10537391490987E-06", "module": "C2"}, {"value": "0.000930704557304097", "module": "C3"}, {"value": "0", "module": "C4"}, {"value": "-0.00966658033021797", "module": "D"}]}, "resolvedFlowVersion": "38.00.000", "flowProperties": [], "typeOfFlow": "Other flow", "classification": {"classHierarchy": "Quantities / Environmental quantities / EPD EN 15804 / LCI indicators", "name": "GaBiCategories"}}, {"dataSetInternalID": 14, "referenceToFlowDataSet": {"shortDescription": [{"value": "Components for re-use (CRU)", "lang": "en"}, {"value": "Komponenten für die Wiederverwendung (CRU)", "lang": "de"}], "type": "flow data set", "refObjectId": "a2b32f97-3fc7-4af2-b209-525bc6426f33", "uri": "../flows/a2b32f97-3fc7-4af2-b209-525bc6426f33.xml"}, "exchange direction": "OUTPUT", "other": {"anies": [{"name": "referenceToUnitGroupDataSet", "value": {"shortDescription": [{"value": "kg", "lang": "en"}], "type": "unit group data set", "refObjectId": "ad38d542-3fe9-439d-9b95-2f5f7752acaf", "uri": "../unitgroups/ad38d542-3fe9-439d-9b95-2f5f7752acaf.xml"}}, {"value": "0", "module": "A1-A3"}, {"value": "0", "module": "A4"}, {"value": "0", "module": "A5"}, {"value": "0", "module": "B1"}, {"value": "0", "module": "C1"}, {"value": "0", "module": "C2"}, {"value": "0", "module": "C3"}, {"value": "0", "module": "C4"}, {"value": "0", "module": "D"}]}, "resolvedFlowVersion": "38.00.000", "flowProperties": [], "typeOfFlow": "Other flow", "classification": {"classHierarchy": "Quantities / Environmental quantities / EPD EN 15804 / LCI indicators", "name": "GaBiCategories"}}, {"dataSetInternalID": 15, "referenceToFlowDataSet": {"shortDescription": [{"value": "Materials for recycling (MFR)", "lang": "en"}, {"value": "Stoffe zum Recycling (MFR)", "lang": "de"}], "type": "flow data set", "refObjectId": "d7fe48a5-4103-49c8-9aae-b0b5dfdbd6ae", "uri": "../flows/d7fe48a5-4103-49c8-9aae-b0b5dfdbd6ae.xml"}, "exchange direction": "OUTPUT", "other": {"anies": [{"name": "referenceToUnitGroupDataSet", "value": {"shortDescription": [{"value": "kg", "lang": "en"}], "type": "unit group data set", "refObjectId": "ad38d542-3fe9-439d-9b95-2f5f7752acaf", "uri": "../unitgroups/ad38d542-3fe9-439d-9b95-2f5f7752acaf.xml"}}, {"value": "0.124", "module": "A1-A3"}, {"value": "0", "module": "A4"}, {"value": "0", "module": "A5"}, {"value": "0", "module": "B1"}, {"value": "0", "module": "C1"}, {"value": "0", "module": "C2"}, {"value": "0.02", "module": "C3"}, {"value": "0", "module": "C4"}, {"value": "0", "module": "D"}]}, "resolvedFlowVersion": "38.00.000", "flowProperties": [], "typeOfFlow": "Other flow", "classification": {"classHierarchy": "Quantities / Environmental quantities / EPD EN 15804 / LCI indicators", "name": "GaBiCategories"}}, {"dataSetInternalID": 16, "referenceToFlowDataSet": {"shortDescription": [{"value": "Materials for energy recovery (MER)", "lang": "en"}, {"value": "Stoffe für die Energierückgewinnung (MER)", "lang": "de"}], "type": "flow data set", "refObjectId": "59a9181c-3aaf-46ee-8b13-2b3723b6e447", "uri": "../flows/59a9181c-3aaf-46ee-8b13-2b3723b6e447.xml"}, "exchange direction": "OUTPUT", "other": {"anies": [{"name": "referenceToUnitGroupDataSet", "value": {"shortDescription": [{"value": "kg", "lang": "en"}], "type": "unit group data set", "refObjectId": "ad38d542-3fe9-439d-9b95-2f5f7752acaf", "uri": "../unitgroups/ad38d542-3fe9-439d-9b95-2f5f7752acaf.xml"}}, {"value": "0", "module": "A1-A3"}, {"value": "0", "module": "A4"}, {"value": "0", "module": "A5"}, {"value": "0", "module": "B1"}, {"value": "0", "module": "C1"}, {"value": "0", "module": "C2"}, {"value": "0", "module": "C3"}, {"value": "0", "module": "C4"}, {"value": "0", "module": "D"}]}, "resolvedFlowVersion": "38.00.000", "flowProperties": [], "typeOfFlow": "Other flow", "classification": {"classHierarchy": "Quantities / Environmental quantities / EPD EN 15804 / LCI indicators", "name": "GaBiCategories"}}, {"dataSetInternalID": 17, "referenceToFlowDataSet": {"shortDescription": [{"value": "Exported electrical energy (EEE)", "lang": "en"}, {"value": "Exportierte elektrische Energie (EEE)", "lang": "de"}], "type": "flow data set", "refObjectId": "4da0c987-2b76-40d6-9e9e-82a017aaaf29", "uri": "../flows/4da0c987-2b76-40d6-9e9e-82a017aaaf29.xml"}, "exchange direction": "OUTPUT", "other": {"anies": [{"name": "referenceToUnitGroupDataSet", "value": {"shortDescription": [{"value": "MJ", "lang": "en"}], "type": "unit group data set", "refObjectId": "93a60a57-a3c8-11da-a746-0800200c9a66", "uri": "../unitgroups/93a60a57-a3c8-11da-a746-0800200c9a66.xml"}}, {"value": "0", "module": "A1-A3"}, {"value": "0", "module": "A4"}, {"value": "5.16933320825969", "module": "A5"}, {"value": "0", "module": "B1"}, {"value": "0", "module": "C1"}, {"value": "0", "module": "C2"}, {"value": "27.34114994499", "module": "C3"}, {"value": "0", "module": "C4"}, {"value": "0", "module": "D"}]}, "resolvedFlowVersion": "38.00.000", "flowProperties": [], "typeOfFlow": "Other flow", "classification": {"classHierarchy": "Quantities / Environmental quantities / EPD EN 15804 / LCI indicators", "name": "GaBiCategories"}}, {"dataSetInternalID": 18, "referenceToFlowDataSet": {"shortDescription": [{"value": "Exported thermal energy (EET)", "lang": "en"}, {"value": "Exportierte thermische Energie (EET)", "lang": "de"}], "type": "flow data set", "refObjectId": "98daf38a-7a79-46d3-9a37-2b7bd0955810", "uri": "../flows/98daf38a-7a79-46d3-9a37-2b7bd0955810.xml"}, "exchange direction": "OUTPUT", "other": {"anies": [{"name": "referenceToUnitGroupDataSet", "value": {"shortDescription": [{"value": "MJ", "lang": "en"}], "type": "unit group data set", "refObjectId": "93a60a57-a3c8-11da-a746-0800200c9a66", "uri": "../unitgroups/93a60a57-a3c8-11da-a746-0800200c9a66.xml"}}, {"value": "0", "module": "A1-A3"}, {"value": "0", "module": "A4"}, {"value": "9.27832031711653", "module": "A5"}, {"value": "0", "module": "B1"}, {"value": "0", "module": "C1"}, {"value": "0", "module": "C2"}, {"value": "49.7192561836308", "module": "C3"}, {"value": "0", "module": "C4"}, {"value": "0", "module": "D"}]}, "resolvedFlowVersion": "38.00.000", "flowProperties": [], "typeOfFlow": "Other flow", "classification": {"classHierarchy": "Quantities / Environmental quantities / EPD EN 15804 / LCI indicators", "name": "GaBiCategories"}}]}, "LCIAResults": {"LCIAResult": [{"referenceToLCIAMethodDataSet": {"shortDescription": [{"value": "Global Warming Potential total (GWP-total)", "lang": "en"}, {"value": "Globales Erwärmungspotenzial total (GWP-total)", "lang": "de"}], "type": "LCIA method data set", "refObjectId": "6a37f984-a4b3-458a-a20a-64418c145fa2", "uri": "../lciamethods/6a37f984-a4b3-458a-a20a-64418c145fa2.xml"}, "other": {"anies": [{"name": "referenceToUnitGroupDataSet", "value": {"shortDescription": [{"value": "kg CO_(2) eq", "lang": "en"}], "type": "unit group data set", "refObjectId": "1ebf3012-d0db-4de2-aefd-ef30cedb0be1", "uri": "../unitgroups/1ebf3012-d0db-4de2-aefd-ef30cedb0be1.xml"}}, {"value": "9.01038979559013", "module": "A1-A3"}, {"value": "0.960763115667233", "module": "A4"}, {"value": "2.57111937861864", "module": "A5"}, {"value": "0", "module": "B1"}, {"value": "0", "module": "C1"}, {"value": "0.0449117521751678", "module": "C2"}, {"value": "25.9870808372895", "module": "C3"}, {"value": "0", "module": "C4"}, {"value": "-6.85342953251944", "module": "D"}]}}, {"referenceToLCIAMethodDataSet": {"shortDescription": [{"value": "Global Warming Potential fossil fuels (GWP-fossil)", "lang": "en"}, {"value": "Globales Erwärmungspotenzial fossil (GWP-fossil)", "lang": "de"}], "type": "LCIA method data set", "refObjectId": "5f635281-343e-44fb-83df-1971b155e6b6", "uri": "../lciamethods/5f635281-343e-44fb-83df-1971b155e6b6.xml"}, "other": {"anies": [{"name": "referenceToUnitGroupDataSet", "value": {"shortDescription": [{"value": "kg CO_(2) eq", "lang": "en"}], "type": "unit group data set", "refObjectId": "1ebf3012-d0db-4de2-aefd-ef30cedb0be1", "uri": "../unitgroups/1ebf3012-d0db-4de2-aefd-ef30cedb0be1.xml"}}, {"value": "22.9132969959578", "module": "A1-A3"}, {"value": "0.950267694344644", "module": "A4"}, {"value": "1.00582854210533", "module": "A5"}, {"value": "0", "module": "B1"}, {"value": "0", "module": "C1"}, {"value": "0.0444211340886411", "module": "C2"}, {"value": "14.0384147487725", "module": "C3"}, {"value": "0", "module": "C4"}, {"value": "-6.82319195511776", "module": "D"}]}}, {"referenceToLCIAMethodDataSet": {"shortDescription": [{"value": "Global Warming Potential biogenic (GWP-biogenic)", "lang": "en"}, {"value": "Globales Erwärmungspotenzial biogen (GWP-biogenic)", "lang": "de"}], "type": "LCIA method data set", "refObjectId": "2356e1ab-0185-4db5-86e5-16de51c7485c", "uri": "../lciamethods/2356e1ab-0185-4db5-86e5-16de51c7485c.xml"}, "other": {"anies": [{"name": "referenceToUnitGroupDataSet", "value": {"shortDescription": [{"value": "kg CO_(2) eq", "lang": "en"}], "type": "unit group data set", "refObjectId": "1ebf3012-d0db-4de2-aefd-ef30cedb0be1", "uri": "../unitgroups/1ebf3012-d0db-4de2-aefd-ef30cedb0be1.xml"}}, {"value": "-13.9221204089352", "module": "A1-A3"}, {"value": "0.00398218018606055", "module": "A4"}, {"value": "1.56491234442207", "module": "A5"}, {"value": "0", "module": "B1"}, {"value": "0", "module": "C1"}, {"value": "0.000186150661611327", "module": "C2"}, {"value": "11.9475487317145", "module": "C3"}, {"value": "0", "module": "C4"}, {"value": "-0.0294416972160291", "module": "D"}]}}, {"referenceToLCIAMethodDataSet": {"shortDescription": [{"value": "Global Warming Potential luluc (GWP-luluc)", "lang": "en"}, {"value": "Globales Erwärmungspotenzial luluc (GWP-luluc)", "lang": "de"}], "type": "LCIA method data set", "refObjectId": "4331bbdb-978a-490d-8707-eeb047f01a55", "uri": "../lciamethods/4331bbdb-978a-490d-8707-eeb047f01a55.xml"}, "other": {"anies": [{"name": "referenceToUnitGroupDataSet", "value": {"shortDescription": [{"value": "kg CO_(2) eq", "lang": "en"}], "type": "unit group data set", "refObjectId": "1ebf3012-d0db-4de2-aefd-ef30cedb0be1", "uri": "../unitgroups/1ebf3012-d0db-4de2-aefd-ef30cedb0be1.xml"}}, {"value": "0.0192132085673827", "module": "A1-A3"}, {"value": "0.00651324113652867", "module": "A4"}, {"value": "0.000378492091222859", "module": "A5"}, {"value": "0", "module": "B1"}, {"value": "0", "module": "C1"}, {"value": "0.000304467424915385", "module": "C2"}, {"value": "0.00111735680249304", "module": "C3"}, {"value": "0", "module": "C4"}, {"value": "-0.000795880185641629", "module": "D"}]}}, {"referenceToLCIAMethodDataSet": {"shortDescription": [{"value": "Depletion potential of the stratospheric ozone layer (ODP)", "lang": "en"}, {"value": "Abbau Potential der stratosphärischen Ozonschicht (ODP)", "lang": "de"}], "type": "LCIA method data set", "refObjectId": "b5c629d6-def3-11e6-bf01-fe55135034f3", "uri": "../lciamethods/b5c629d6-def3-11e6-bf01-fe55135034f3.xml"}, "other": {"anies": [{"name": "referenceToUnitGroupDataSet", "value": {"shortDescription": [{"value": "kg CFC11 eq", "lang": "en"}], "type": "unit group data set", "refObjectId": "d9e957c9-7309-4474-bf3a-7777df6c4e5b", "uri": "../unitgroups/d9e957c9-7309-4474-bf3a-7777df6c4e5b.xml"}}, {"value": "3.31014363963425E-10", "module": "A1-A3"}, {"value": "9.49172970690696E-14", "module": "A4"}, {"value": "2.98148006196777E-12", "module": "A5"}, {"value": "0", "module": "B1"}, {"value": "0", "module": "C1"}, {"value": "4.43699602283579E-15", "module": "C2"}, {"value": "1.43573677397693E-11", "module": "C3"}, {"value": "0", "module": "C4"}, {"value": "-4.89055756974152E-11", "module": "D"}]}}, {"referenceToLCIAMethodDataSet": {"shortDescription": [{"value": "Acidification potential of land and water (AP)", "lang": "en"}, {"value": "Versauerungspotenzial von Boden und Wasser (AP)", "lang": "de"}], "type": "LCIA method data set", "refObjectId": "b5c611c6-def3-11e6-bf01-fe55135034f3", "uri": "../lciamethods/b5c611c6-def3-11e6-bf01-fe55135034f3.xml"}, "other": {"anies": [{"name": "referenceToUnitGroupDataSet", "value": {"shortDescription": [{"value": "mol H^(+) eq", "lang": "en"}], "type": "unit group data set", "refObjectId": "42e089ac-92bf-4bf2-8ca1-5fc40d18f2ed", "uri": "../unitgroups/42e089ac-92bf-4bf2-8ca1-5fc40d18f2ed.xml"}}, {"value": "0.058076596967021", "module": "A1-A3"}, {"value": "0.00107966365850088", "module": "A4"}, {"value": "0.00264758185554386", "module": "A5"}, {"value": "0", "module": "B1"}, {"value": "0", "module": "C1"}, {"value": "5.04698669967687E-05", "module": "C2"}, {"value": "0.006052940310442", "module": "C3"}, {"value": "0", "module": "C4"}, {"value": "-0.00932525198653514", "module": "D"}]}}, {"referenceToLCIAMethodDataSet": {"shortDescription": [{"value": "Eutrophication potential aquatic freshwater (EP-freshwater)", "lang": "en"}, {"value": "Eutrophierungspotenzial Süßwasser (EP-freshwater)", "lang": "de"}], "type": "LCIA method data set", "refObjectId": "b53ec18f-7377-4ad3-86eb-cc3f4f276b2b", "uri": "../lciamethods/b53ec18f-7377-4ad3-86eb-cc3f4f276b2b.xml"}, "other": {"anies": [{"name": "referenceToUnitGroupDataSet", "value": {"shortDescription": [{"value": "kg P eq", "lang": "en"}], "type": "unit group data set", "refObjectId": "0429039d-a61d-4590-ba67-aa4a20a810a1", "uri": "../unitgroups/0429039d-a61d-4590-ba67-aa4a20a810a1.xml"}}, {"value": "0.000219588911556819", "module": "A1-A3"}, {"value": "3.45284150357338E-06", "module": "A4"}, {"value": "1.20385934621149E-06", "module": "A5"}, {"value": "0", "module": "B1"}, {"value": "0", "module": "C1"}, {"value": "1.6140623987311E-07", "module": "C2"}, {"value": "3.71474882026998E-06", "module": "C3"}, {"value": "0", "module": "C4"}, {"value": "-9.78399467307397E-06", "module": "D"}]}}, {"referenceToLCIAMethodDataSet": {"shortDescription": [{"value": "Eutrophication potential aquatic marine (EP-marine)", "lang": "en"}, {"value": "Eutrophierungspotenzial Salzwasser (EP-marine)", "lang": "de"}], "type": "LCIA method data set", "refObjectId": "b5c619fa-def3-11e6-bf01-fe55135034f3", "uri": "../lciamethods/b5c619fa-def3-11e6-bf01-fe55135034f3.xml"}, "other": {"anies": [{"name": "referenceToUnitGroupDataSet", "value": {"shortDescription": [{"value": "kg N eq", "lang": "en"}], "type": "unit group data set", "refObjectId": "d05bb823-ecdf-4686-8c40-bf1d9257859f", "uri": "../unitgroups/d05bb823-ecdf-4686-8c40-bf1d9257859f.xml"}}, {"value": "0.0224844099013065", "module": "A1-A3"}, {"value": "0.000347565154103554", "module": "A4"}, {"value": "0.000682197398170886", "module": "A5"}, {"value": "0", "module": "B1"}, {"value": "0", "module": "C1"}, {"value": "1.62472515974785E-05", "module": "C2"}, {"value": "0.0020744782449316", "module": "C3"}, {"value": "0", "module": "C4"}, {"value": "-0.00231085247699826", "module": "D"}]}}, {"referenceToLCIAMethodDataSet": {"shortDescription": [{"value": "Eutrophication potential terrestrial (EP-terrestrial)", "lang": "en"}, {"value": "Eutrophierungspotenzial Land (EP-terrestrial)", "lang": "de"}], "type": "LCIA method data set", "refObjectId": "b5c614d2-def3-11e6-bf01-fe55135034f3", "uri": "../lciamethods/b5c614d2-def3-11e6-bf01-fe55135034f3.xml"}, "other": {"anies": [{"name": "referenceToUnitGroupDataSet", "value": {"shortDescription": [{"value": "mol N eq", "lang": "en"}], "type": "unit group data set", "refObjectId": "71b4d617-0ec9-4d3f-b65e-e438940c2401", "uri": "../unitgroups/71b4d617-0ec9-4d3f-b65e-e438940c2401.xml"}}, {"value": "0.211892541968433", "module": "A1-A3"}, {"value": "0.00416264530283898", "module": "A4"}, {"value": "0.00803248354066309", "module": "A5"}, {"value": "0", "module": "B1"}, {"value": "0", "module": "C1"}, {"value": "0.000194586668852702", "module": "C2"}, {"value": "0.0258528705031771", "module": "C3"}, {"value": "0", "module": "C4"}, {"value": "-0.0247278913742158", "module": "D"}]}}, {"referenceToLCIAMethodDataSet": {"shortDescription": [{"value": "Formation potential of tropospheric ozone photochemical oxidants (POCP)", "lang": "en"}, {"value": "Bildungspotential für troposphärisches Ozon (POCP)", "lang": "de"}], "type": "LCIA method data set", "refObjectId": "b5c610fe-def3-11e6-bf01-fe55135034f3", "uri": "../lciamethods/b5c610fe-def3-11e6-bf01-fe55135034f3.xml"}, "other": {"anies": [{"name": "referenceToUnitGroupDataSet", "value": {"shortDescription": [{"value": "kg NMVOC eq", "lang": "en"}], "type": "unit group data set", "refObjectId": "d27c25f8-fbc1-44c6-b47b-4adbae4199c6", "uri": "../unitgroups/d27c25f8-fbc1-44c6-b47b-4adbae4199c6.xml"}}, {"value": "0.0622112598591145", "module": "A1-A3"}, {"value": "0.000929673706063141", "module": "A4"}, {"value": "0.00608912427516884", "module": "A5"}, {"value": "0.002981", "module": "B1"}, {"value": "0", "module": "C1"}, {"value": "4.34584492364496E-05", "module": "C2"}, {"value": "0.0057740992195414", "module": "C3"}, {"value": "0", "module": "C4"}, {"value": "-0.00632315471325989", "module": "D"}]}}, {"referenceToLCIAMethodDataSet": {"shortDescription": [{"value": "Abiotic depletion potential for non fossil resources (ADPE)", "lang": "en"}, {"value": "Potenzial für den abiotischen Abbau nicht fossiler Ressourcen (ADPE)", "lang": "de"}], "type": "LCIA method data set", "refObjectId": "b2ad6494-c78d-11e6-9d9d-cec0c932ce01", "uri": "../lciamethods/b2ad6494-c78d-11e6-9d9d-cec0c932ce01.xml"}, "other": {"anies": [{"name": "referenceToUnitGroupDataSet", "value": {"shortDescription": [{"value": "kg Sb eq", "lang": "en"}], "type": "unit group data set", "refObjectId": "54ccd2d9-a32a-4fc2-923d-f2c8c93e89d4", "uri": "../unitgroups/54ccd2d9-a32a-4fc2-923d-f2c8c93e89d4.xml"}}, {"value": "4.13046859899432E-06", "module": "A1-A3"}, {"value": "9.74205143445405E-08", "module": "A4"}, {"value": "5.12964092594709E-06", "module": "A5"}, {"value": "0", "module": "B1"}, {"value": "0", "module": "C1"}, {"value": "4.55401120803935E-09", "module": "C2"}, {"value": "3.51908886888068E-07", "module": "C3"}, {"value": "0", "module": "C4"}, {"value": "-4.44235960124666E-06", "module": "D"}]}}, {"referenceToLCIAMethodDataSet": {"shortDescription": [{"value": "Abiotic depletion potential for fossil resources (ADPF)", "lang": "en"}, {"value": "Potenzial für den abiotischen Abbau fossiler Brennstoffe (ADPF)", "lang": "de"}], "type": "LCIA method data set", "refObjectId": "b2ad6110-c78d-11e6-9d9d-cec0c932ce01", "uri": "../lciamethods/b2ad6110-c78d-11e6-9d9d-cec0c932ce01.xml"}, "other": {"anies": [{"name": "referenceToUnitGroupDataSet", "value": {"shortDescription": [{"value": "MJ", "lang": "en"}], "type": "unit group data set", "refObjectId": "93a60a57-a3c8-11da-a746-0800200c9a66", "uri": "../unitgroups/93a60a57-a3c8-11da-a746-0800200c9a66.xml"}}, {"value": "451.803120534357", "module": "A1-A3"}, {"value": "12.6883110158772", "module": "A4"}, {"value": "8.81060940172172", "module": "A5"}, {"value": "0", "module": "B1"}, {"value": "0", "module": "C1"}, {"value": "0.593126724552466", "module": "C2"}, {"value": "27.5076042800258", "module": "C3"}, {"value": "0", "module": "C4"}, {"value": "-61.9738458581352", "module": "D"}]}}, {"referenceToLCIAMethodDataSet": {"shortDescription": [{"value": "Water use (WDP)", "lang": "en"}, {"value": "Wassernutzung (WDP)", "lang": "de"}], "type": "LCIA method data set", "refObjectId": "b2ad66ce-c78d-11e6-9d9d-cec0c932ce01", "uri": "../lciamethods/b2ad66ce-c78d-11e6-9d9d-cec0c932ce01.xml"}, "other": {"anies": [{"name": "referenceToUnitGroupDataSet", "value": {"shortDescription": [{"value": "m^(3) world eq deprived", "lang": "en"}], "type": "unit group data set", "refObjectId": "6ae2df01-888e-46c8-b17d-49fa3869b476", "uri": "../unitgroups/6ae2df01-888e-46c8-b17d-49fa3869b476.xml"}}, {"value": "2.97410687112953", "module": "A1-A3"}, {"value": "0.0108142354931794", "module": "A4"}, {"value": "0.425757990255486", "module": "A5"}, {"value": "0", "module": "B1"}, {"value": "0", "module": "C1"}, {"value": "0.000505521347055748", "module": "C2"}, {"value": "2.20091233853667", "module": "C3"}, {"value": "0", "module": "C4"}, {"value": "-0.805375675442071", "module": "D"}]}}, {"referenceToLCIAMethodDataSet": {"shortDescription": [{"value": "Incidence of disease due to PM emissions (PM)", "lang": "en"}, {"value": "Auftreten von Krankheiten aufgrund von Feinstaubemissionen (PM)", "lang": "de"}], "type": "LCIA method data set", "refObjectId": "b5c602c6-def3-11e6-bf01-fe55135034f3", "uri": "../lciamethods/b5c602c6-def3-11e6-bf01-fe55135034f3.xml"}, "other": {"anies": [{"name": "referenceToUnitGroupDataSet", "value": {"shortDescription": [{"value": "Disease incidence", "lang": "en"}], "type": "unit group data set", "refObjectId": "3883559b-648f-4afc-8ba2-0bd24f3affa3", "uri": "../unitgroups/3883559b-648f-4afc-8ba2-0bd24f3affa3.xml"}}, {"value": "2.47567029052042E-06", "module": "A1-A3"}, {"value": "7.42138128433623E-09", "module": "A4"}, {"value": "2.20945956581938E-07", "module": "A5"}, {"value": "0", "module": "B1"}, {"value": "0", "module": "C1"}, {"value": "3.4691926824029E-10", "module": "C2"}, {"value": "1.05239894137937E-07", "module": "C3"}, {"value": "0", "module": "C4"}, {"value": "-8.19754970172805E-08", "module": "D"}]}}, {"referenceToLCIAMethodDataSet": {"shortDescription": [{"value": "Human exposure efficiency relative to U235 (IR)", "lang": "en"}, {"value": "Wirkung durch Exposition des Menschen mit U235 (IR)", "lang": "de"}], "type": "LCIA method data set", "refObjectId": "b5c632be-def3-11e6-bf01-fe55135034f3", "uri": "../lciamethods/b5c632be-def3-11e6-bf01-fe55135034f3.xml"}, "other": {"anies": [{"name": "referenceToUnitGroupDataSet", "value": {"shortDescription": [{"value": "kBq U235 eq", "lang": "en"}], "type": "unit group data set", "refObjectId": "456b05bf-1415-44a9-9993-02452f554c09", "uri": "../unitgroups/456b05bf-1415-44a9-9993-02452f554c09.xml"}}, {"value": "4.54236647568194", "module": "A1-A3"}, {"value": "0.00357049018880274", "module": "A4"}, {"value": "0.0748047742995416", "module": "A5"}, {"value": "0", "module": "B1"}, {"value": "0", "module": "C1"}, {"value": "0.000166905835463939", "module": "C2"}, {"value": "0.11025612473744", "module": "C3"}, {"value": "0", "module": "C4"}, {"value": "-1.63757586877028", "module": "D"}]}}, {"referenceToLCIAMethodDataSet": {"shortDescription": [{"value": "Comparative toxic unit for ecosystems (ETP-fw)", "lang": "en"}, {"value": "Toxizitätsvergleichseinheit für Ökosysteme (ETP-fw)", "lang": "de"}], "type": "LCIA method data set", "refObjectId": "ee1082d1-b0f7-43ca-a1f0-21e2a4a74511", "uri": "../lciamethods/ee1082d1-b0f7-43ca-a1f0-21e2a4a74511.xml"}, "other": {"anies": [{"name": "referenceToUnitGroupDataSet", "value": {"shortDescription": [{"value": "CTUe", "lang": "en"}], "type": "unit group data set", "refObjectId": "aa959ded-f1eb-4efb-9c5c-2d60be36b3e6", "uri": "../unitgroups/aa959ded-f1eb-4efb-9c5c-2d60be36b3e6.xml"}}, {"value": "180.793787869821", "module": "A1-A3"}, {"value": "8.99147234478569", "module": "A4"}, {"value": "4.66658228331774", "module": "A5"}, {"value": "0.45643654065", "module": "B1"}, {"value": "0", "module": "C1"}, {"value": "0.420314613512658", "module": "C2"}, {"value": "22.1201854073357", "module": "C3"}, {"value": "0", "module": "C4"}, {"value": "-27.4339943593604", "module": "D"}]}}, {"referenceToLCIAMethodDataSet": {"shortDescription": [{"value": "Comparative toxic unit for humans (carcinogenic) (HTP-c)", "lang": "en"}, {"value": "Toxizitätsvergleichseinheit für Menschen (krebserregend) (HTP-c)", "lang": "de"}], "type": "LCIA method data set", "refObjectId": "2299222a-bbd8-474f-9d4f-4dd1f18aea7c", "uri": "../lciamethods/2299222a-bbd8-474f-9d4f-4dd1f18aea7c.xml"}, "other": {"anies": [{"name": "referenceToUnitGroupDataSet", "value": {"shortDescription": [{"value": "CTUh", "lang": "en"}], "type": "unit group data set", "refObjectId": "d4c9523e-2d7e-49fd-8469-998f547d3a70", "uri": "../unitgroups/d4c9523e-2d7e-49fd-8469-998f547d3a70.xml"}}, {"value": "1.92150608349496E-08", "module": "A1-A3"}, {"value": "1.85346244624982E-10", "module": "A4"}, {"value": "3.12971657738948E-08", "module": "A5"}, {"value": "3.304E-08", "module": "B1"}, {"value": "0", "module": "C1"}, {"value": "8.66418003506954E-12", "module": "C2"}, {"value": "8.99343903481971E-10", "module": "C3"}, {"value": "0", "module": "C4"}, {"value": "-1.30135358855738E-09", "module": "D"}]}}, {"referenceToLCIAMethodDataSet": {"shortDescription": [{"value": "Comparative toxic unit for humans (noncarcinogenic) (HTP-nc)", "lang": "en"}, {"value": "Toxizitätsvergleichseinheit für Menschen (nicht krebserregend) (HTP-nc)", "lang": "de"}], "type": "LCIA method data set", "refObjectId": "3af763a5-b7a1-48c9-9cee-1f223481fcef", "uri": "../lciamethods/3af763a5-b7a1-48c9-9cee-1f223481fcef.xml"}, "other": {"anies": [{"name": "referenceToUnitGroupDataSet", "value": {"shortDescription": [{"value": "CTUh", "lang": "en"}], "type": "unit group data set", "refObjectId": "d4c9523e-2d7e-49fd-8469-998f547d3a70", "uri": "../unitgroups/d4c9523e-2d7e-49fd-8469-998f547d3a70.xml"}}, {"value": "2.58103842542652E-07", "module": "A1-A3"}, {"value": "1.00546770643489E-08", "module": "A4"}, {"value": "2.31524213259189E-08", "module": "A5"}, {"value": "4.58008661E-10", "module": "B1"}, {"value": "0", "module": "C1"}, {"value": "4.70015092327698E-10", "module": "C2"}, {"value": "9.15079746837281E-08", "module": "C3"}, {"value": "0", "module": "C4"}, {"value": "-2.95302535707626E-08", "module": "D"}]}}, {"referenceToLCIAMethodDataSet": {"shortDescription": [{"value": "Soil quality index (SQP)", "lang": "en"}, {"value": "Bodenqualitätsindex (SQP)", "lang": "de"}], "type": "LCIA method data set", "refObjectId": "b2ad6890-c78d-11e6-9d9d-cec0c932ce01", "uri": "../lciamethods/b2ad6890-c78d-11e6-9d9d-cec0c932ce01.xml"}, "other": {"anies": [{"name": "referenceToUnitGroupDataSet", "value": {"shortDescription": [{"value": "SQP", "lang": "en"}], "type": "unit group data set", "refObjectId": "f130951c-e67f-4f7f-8dd4-665de3974e18", "uri": "../unitgroups/f130951c-e67f-4f7f-8dd4-665de3974e18.xml"}}, {"value": "2916.60792575429", "module": "A1-A3"}, {"value": "5.37099426195297", "module": "A4"}, {"value": "261.673940581776", "module": "A5"}, {"value": "0", "module": "B1"}, {"value": "0", "module": "C1"}, {"value": "0.251072048139105", "module": "C2"}, {"value": "6.44890886422084", "module": "C3"}, {"value": "0", "module": "C4"}, {"value": "-21.9458836597928", "module": "D"}]}}]}, "otherAttributes": {"{http://www.indata.network/EPD/2019}epd-version": "1.2"}, "version": "1.1", "locations": "../ILCDLocations.xml"}