{"processInformation": {"dataSetInformation": {"UUID": "5c85c594-5d7d-4cfa-b9e7-0270c3ad1ffd", "name": {"baseName": [{"value": "Butt welded Fittings (DÖLING Fittings GmbH & CO KG)", "lang": "en"}]}, "synonyms": [{"value": "Butt welded Fittings (DÖLING Fittings GmbH & CO KG)", "lang": "en"}], "classificationInformation": {"classification": [{"class": [{"value": "Metalle", "level": 0, "classId": "4"}, {"value": "Edelstahl", "level": 1, "classId": "4.2"}, {"value": "Edelstahl Trinkwasserrohre", "level": 2, "classId": "4.2.03"}], "name": "OEKOBAU.DAT"}]}, "generalComment": [{"value": "The owner of this EPD shall be liable for the underlying information and evidence. The programme operator Kiwa-Ecobility Experts shall not be liable with respect to manufacturer data, life cycle assessment data and evidence.\r\nThis is a Cradle to gate with modules C1-C4 and module D EPD.\r\n", "lang": "en"}], "other": {"anies": [{"scenario": [{"description": [{"value": "It is assumed that the disassembly for the de-construction is carried out manually by hand, which leads to no processes being added to the module C1. The NMD is the Netherlands’ national environmental database, providing standardized data for assessing the environmental impact of building materials. The NMD waste scenario for \"Steel, piping civil constructions (NMD ID 72)\" is considered representative for the life cycle of Butt welded Fittings and used in the calculation. The process \"Scrap steel {Europe without Switzerland}| treatment of scrap steel, inert material landfill\" is used for landfilling and To be left, whereby the dataset \"Materials for recycling, no waste processing taken into account\" is used for recycling. The recycled waste is reused as benefits in the process \"World Steel method (Steel production, electric, low-alloyed - Steel production, converter, unalloyed)\".", "lang": "en"}], "name": "Standard Scenarios", "default": true}]}, "<ns11:modules xmlns:ns11=\"http://openlca.org/epd_ilcd\" xmlns=\"http://lca.jrc.it/ILCD/Process\" xmlns:c=\"http://lca.jrc.it/ILCD/Contact\" xmlns:common=\"http://lca.jrc.it/ILCD/Common\" xmlns:epd=\"http://www.iai.kit.edu/EPD/2013\" xmlns:epd2=\"http://www.indata.network/EPD/2019\" xmlns:f=\"http://lca.jrc.it/ILCD/Flow\" xmlns:fp=\"http://lca.jrc.it/ILCD/FlowProperty\" xmlns:m=\"http://lca.jrc.it/ILCD/LCIAMethod\" xmlns:s=\"http://lca.jrc.it/ILCD/Source\" xmlns:u=\"http://lca.jrc.it/ILCD/UnitGroup\" name=\"A1\" scenario=\"Standard Scenarios\"/>", "<ns11:modules xmlns:ns11=\"http://openlca.org/epd_ilcd\" xmlns=\"http://lca.jrc.it/ILCD/Process\" xmlns:c=\"http://lca.jrc.it/ILCD/Contact\" xmlns:common=\"http://lca.jrc.it/ILCD/Common\" xmlns:epd=\"http://www.iai.kit.edu/EPD/2013\" xmlns:epd2=\"http://www.indata.network/EPD/2019\" xmlns:f=\"http://lca.jrc.it/ILCD/Flow\" xmlns:fp=\"http://lca.jrc.it/ILCD/FlowProperty\" xmlns:m=\"http://lca.jrc.it/ILCD/LCIAMethod\" xmlns:s=\"http://lca.jrc.it/ILCD/Source\" xmlns:u=\"http://lca.jrc.it/ILCD/UnitGroup\" name=\"A2\" scenario=\"Standard Scenarios\"/>", "<ns11:modules xmlns:ns11=\"http://openlca.org/epd_ilcd\" xmlns=\"http://lca.jrc.it/ILCD/Process\" xmlns:c=\"http://lca.jrc.it/ILCD/Contact\" xmlns:common=\"http://lca.jrc.it/ILCD/Common\" xmlns:epd=\"http://www.iai.kit.edu/EPD/2013\" xmlns:epd2=\"http://www.indata.network/EPD/2019\" xmlns:f=\"http://lca.jrc.it/ILCD/Flow\" xmlns:fp=\"http://lca.jrc.it/ILCD/FlowProperty\" xmlns:m=\"http://lca.jrc.it/ILCD/LCIAMethod\" xmlns:s=\"http://lca.jrc.it/ILCD/Source\" xmlns:u=\"http://lca.jrc.it/ILCD/UnitGroup\" name=\"A3\" scenario=\"Standard Scenarios\"/>", "<ns11:modules xmlns:ns11=\"http://openlca.org/epd_ilcd\" xmlns=\"http://lca.jrc.it/ILCD/Process\" xmlns:c=\"http://lca.jrc.it/ILCD/Contact\" xmlns:common=\"http://lca.jrc.it/ILCD/Common\" xmlns:epd=\"http://www.iai.kit.edu/EPD/2013\" xmlns:epd2=\"http://www.indata.network/EPD/2019\" xmlns:f=\"http://lca.jrc.it/ILCD/Flow\" xmlns:fp=\"http://lca.jrc.it/ILCD/FlowProperty\" xmlns:m=\"http://lca.jrc.it/ILCD/LCIAMethod\" xmlns:s=\"http://lca.jrc.it/ILCD/Source\" xmlns:u=\"http://lca.jrc.it/ILCD/UnitGroup\" name=\"A1-A3\" scenario=\"Standard Scenarios\"/>", "<ns11:modules xmlns:ns11=\"http://openlca.org/epd_ilcd\" xmlns=\"http://lca.jrc.it/ILCD/Process\" xmlns:c=\"http://lca.jrc.it/ILCD/Contact\" xmlns:common=\"http://lca.jrc.it/ILCD/Common\" xmlns:epd=\"http://www.iai.kit.edu/EPD/2013\" xmlns:epd2=\"http://www.indata.network/EPD/2019\" xmlns:f=\"http://lca.jrc.it/ILCD/Flow\" xmlns:fp=\"http://lca.jrc.it/ILCD/FlowProperty\" xmlns:m=\"http://lca.jrc.it/ILCD/LCIAMethod\" xmlns:s=\"http://lca.jrc.it/ILCD/Source\" xmlns:u=\"http://lca.jrc.it/ILCD/UnitGroup\" name=\"C1\" scenario=\"Standard Scenarios\"/>", "<ns11:modules xmlns:ns11=\"http://openlca.org/epd_ilcd\" xmlns=\"http://lca.jrc.it/ILCD/Process\" xmlns:c=\"http://lca.jrc.it/ILCD/Contact\" xmlns:common=\"http://lca.jrc.it/ILCD/Common\" xmlns:epd=\"http://www.iai.kit.edu/EPD/2013\" xmlns:epd2=\"http://www.indata.network/EPD/2019\" xmlns:f=\"http://lca.jrc.it/ILCD/Flow\" xmlns:fp=\"http://lca.jrc.it/ILCD/FlowProperty\" xmlns:m=\"http://lca.jrc.it/ILCD/LCIAMethod\" xmlns:s=\"http://lca.jrc.it/ILCD/Source\" xmlns:u=\"http://lca.jrc.it/ILCD/UnitGroup\" name=\"C2\" scenario=\"Standard Scenarios\"/>", "<ns11:modules xmlns:ns11=\"http://openlca.org/epd_ilcd\" xmlns=\"http://lca.jrc.it/ILCD/Process\" xmlns:c=\"http://lca.jrc.it/ILCD/Contact\" xmlns:common=\"http://lca.jrc.it/ILCD/Common\" xmlns:epd=\"http://www.iai.kit.edu/EPD/2013\" xmlns:epd2=\"http://www.indata.network/EPD/2019\" xmlns:f=\"http://lca.jrc.it/ILCD/Flow\" xmlns:fp=\"http://lca.jrc.it/ILCD/FlowProperty\" xmlns:m=\"http://lca.jrc.it/ILCD/LCIAMethod\" xmlns:s=\"http://lca.jrc.it/ILCD/Source\" xmlns:u=\"http://lca.jrc.it/ILCD/UnitGroup\" name=\"C3\" scenario=\"Standard Scenarios\"/>", "<ns11:modules xmlns:ns11=\"http://openlca.org/epd_ilcd\" xmlns=\"http://lca.jrc.it/ILCD/Process\" xmlns:c=\"http://lca.jrc.it/ILCD/Contact\" xmlns:common=\"http://lca.jrc.it/ILCD/Common\" xmlns:epd=\"http://www.iai.kit.edu/EPD/2013\" xmlns:epd2=\"http://www.indata.network/EPD/2019\" xmlns:f=\"http://lca.jrc.it/ILCD/Flow\" xmlns:fp=\"http://lca.jrc.it/ILCD/FlowProperty\" xmlns:m=\"http://lca.jrc.it/ILCD/LCIAMethod\" xmlns:s=\"http://lca.jrc.it/ILCD/Source\" xmlns:u=\"http://lca.jrc.it/ILCD/UnitGroup\" name=\"C4\" scenario=\"Standard Scenarios\"/>", "<ns11:modules xmlns:ns11=\"http://openlca.org/epd_ilcd\" xmlns=\"http://lca.jrc.it/ILCD/Process\" xmlns:c=\"http://lca.jrc.it/ILCD/Contact\" xmlns:common=\"http://lca.jrc.it/ILCD/Common\" xmlns:epd=\"http://www.iai.kit.edu/EPD/2013\" xmlns:epd2=\"http://www.indata.network/EPD/2019\" xmlns:f=\"http://lca.jrc.it/ILCD/Flow\" xmlns:fp=\"http://lca.jrc.it/ILCD/FlowProperty\" xmlns:m=\"http://lca.jrc.it/ILCD/LCIAMethod\" xmlns:s=\"http://lca.jrc.it/ILCD/Source\" xmlns:u=\"http://lca.jrc.it/ILCD/UnitGroup\" name=\"D\" scenario=\"Standard Scenarios\"/>"]}}, "quantitativeReference": {"referenceToReferenceFlow": [1], "type": "Reference flow(s)"}, "time": {"referenceYear": 2023, "dataSetValidUntil": 2030, "timeRepresentativenessDescription": [{"value": "All process-specific data was collected for the 2023 operating year from 01.01.2023 to 31.12.2023. ", "lang": "en"}], "other": {"anies": [{"name": "publicationDateOfEPD", "value": 1742169600000}]}}, "geography": {"locationOfOperationSupplyOrProduction": {"descriptionOfRestrictions": [{"value": "The reference area is Germany. \r", "lang": "en"}], "location": "DE"}}, "technology": {"technologyDescriptionAndIncludedProcesses": [{"value": "This EPD is an average EPD. This approach was chosen due to many different product sizes being available, which all require a different number of processing steps. The EPD includes weld fittings made of seamless steel pipes. The product portfolio consists of tees, concentric and eccentric reducers, saddles and flange tube ends. The products covered in this EPD are classified and traded under the following TARif Intégré Communautaire (TARIC): HS Code 73079319. TEEs: These products are pipe fittings in the shape of a “T”. They allow three pipes to be connected, creating a main pipe and a branch.  Concentric reducers: These special pipe fittings are used in piping systems to connect two pipes with different diameters where the center points of the pipes are on the same axis.  Eccentric reducers: These special pipe fittings are used in piping systems to connect two pipes with different diameters, where the center points of the pipes are not on the same axis but are offset to one another. Flange tube ends: These special pipe fittings are used in piping systems to enable a flange to be connected to the pipe. In the process, parts of a pipe are flanged and thus create a contact surface for the flange. Saddle fittings: A steel saddle fitting is a pipe fitting used to create a branch from a main line. The saddle fitting usually has one side that is welded onto a pipe and one open side that opens into another pipe or fitting.  For the placing on the market in the European Union/European Free Trade Association (EU/EFTA) (with the exception of Switzerland) the following legal provisions apply: 2014/68/ EU of the European Parliament and of the Council of 15 May 2014 on the harmonization of the laws of the Member States relating to the making available on the market of pressure equipment and the harmonized standards based on these provisions: • EN 10253-1:2000, Butt-welding pipe fittings – Part 1: Wrought carbon steel for general use and without specific inspection requirements • EN 10253-2:2021, Butt-welding pipe fittings – Part 2: Non alloy and ferritic alloy steels with specific inspection. First, a steel pipe is transported internally by crane and trolley. The pipe is then sawn into the desired length and cold or hot formed several times depending on the exact product and size. Some of the forming processes may use water. The next step consists of a heat treatment. Finally it is shot blasted to clean and treat its surface and readying it for the end finishing. Lastly, the product is labeled and put into storage until it is being transported to the customer.", "lang": "en"}], "technologicalApplicability": [{"value": "The areas of application are diverse and include all applications in which media such as liquids, gases or vapors are transported through pipelines. These include pipeline construction, the chemical industry, the oil and gas industry, mechanical engineering and power generation. Weld fittings are used to adjust the pressure or flow of the medium in the pipeline. For example, pressure losses can be compensated without causing turbulence or a disruption in the flow. Flange tube ends create the contact surface for a flange.", "lang": "en"}], "referenceToTechnologyFlowDiagrammOrPicture": [{"shortDescription": [{"value": "Flow Chart for Butt welded Fittings ", "lang": "en"}], "type": "source data set", "refObjectId": "6716b8d0-3f35-44e9-9966-41f941a128ff", "version": "00.00.001"}]}}, "modellingAndValidation": {"LCIMethodAndAllocation": {"typeOfDataSet": "EPD", "other": {"anies": [{"name": "subType", "value": "average dataset"}]}}, "dataSourcesTreatmentAndRepresentativeness": {"referenceToDataSource": [{"shortDescription": [{"value": "ecoinvent 3.6 database", "lang": "en"}], "type": "source data set", "refObjectId": "766b9973-5ee8-48a2-8098-72c8e20b369f", "version": "00.00.001"}, {"shortDescription": [{"value": "ecoinvent database (general)", "lang": "en"}], "type": "source data set", "refObjectId": "b497a91f-e14b-4b69-8f28-f50eb1576766", "version": "00.03.002"}], "useAdviceForDataSet": [{"value": "The areas of application are diverse and include all applications in which media such as liquids, gases or vapors are transported through pipelines. These include pipeline construction, the chemical industry, the oil and gas industry, mechanical engineering and power generation. Weld fittings are used to adjust the pressure or flow of the medium in the pipeline. For example, pressure losses can be compensated without causing turbulence or a disruption in the flow. Flange tube ends create the contact surface for a flange.", "lang": "en"}], "other": {"anies": [{"name": "referenceToOriginalEPD", "value": {"shortDescription": {"value": "EPD for Butt welded Fittings ", "defaultValue": "EPD for Butt welded Fittings ", "lstrings": [{"lang": "en", "value": "EPD for Butt welded Fittings "}]}, "version": {"version": 1, "majorVersion": 0, "minorVersion": 0, "subMinorVersion": 1, "zero": false, "versionString": "00.00.001"}, "type": "source data set", "uuid": {"uuid": "6591b8c2-74e7-4d98-aff8-503c84eca50d"}, "refObjectId": "6591b8c2-74e7-4d98-aff8-503c84eca50d", "versionAsString": "00.00.001", "resourceURLs": ["https://oekobaudat.de/OEKOBAU.DAT/resource/sources/6591b8c2-74e7-4d98-aff8-503c84eca50d/93584-butt-welded-fittings--202503170536-long.pdf?version=00.00.001"]}}]}}, "validation": {"review": [{"reviewDetails": [{"value": "The independent verification is in accordance with the ISO 14025:2011. ", "lang": "en"}], "referenceToNameOfReviewerAndInstitution": [{"shortDescription": [{"value": "Gaurav Das", "lang": "en"}], "type": "contact data set", "refObjectId": "698a18c3-0b47-4b75-b1c1-7e278cb44743", "version": "00.00.001"}], "type": "Independent external review"}]}, "complianceDeclarations": {"compliance": [{"referenceToComplianceSystem": {"shortDescription": [{"value": "ISO 14025", "lang": "en"}], "type": "source data set", "refObjectId": "4f2eb655-6e44-4874-a95a-e28f5442cd4d", "version": "00.00.001"}}, {"referenceToComplianceSystem": {"shortDescription": [{"value": "EN 15804+A2 (EF 3.0)", "lang": "de"}, {"value": "EN 15804+A2 (EF 3.0)", "lang": "en"}], "type": "source data set", "refObjectId": "c0016b33-8cf7-415c-ac6e-deba0d21440d", "version": "00.02.000"}}]}}, "administrativeInformation": {"commissionerAndGoal": {"referenceToCommissioner": [{"shortDescription": [{"value": "DÖLING Fittings GmbH & Co. KG", "lang": "en"}], "type": "contact data set", "refObjectId": "dcb30f4a-8963-40e4-ab47-6a038a653595", "version": "00.00.001"}]}, "dataGenerator": {"referenceToPersonOrEntityGeneratingTheDataSet": [{"shortDescription": [{"value": "Kiwa GmbH (Berlin)", "lang": "en"}], "type": "contact data set", "refObjectId": "3ea4a87a-3f88-4633-b7e7-1bbdd272be43", "version": "00.00.002"}]}, "dataEntryBy": {"timeStamp": 1742820226376, "referenceToDataSetFormat": [{"shortDescription": [{"value": "ILCD format", "lang": "en"}], "type": "source data set", "refObjectId": "a97a0155-0234-4b87-b4ce-a45da52f2a40", "version": "01.00.000", "uri": "http://lca.jrc.ec.europa.eu/lcainfohub/sample_data/ilcd/sources/ILCD_Format_a97a0155-0234-4b87-b4ce-a45da52f2a40_01.00.000.xml"}, {"shortDescription": [{"value": "EPD Data Format Extensions v1.2", "lang": "en"}, {"value": "EPD-Datenformaterweiterungen v1.2", "lang": "de"}], "type": "source data set", "refObjectId": "a29449fd-aa2f-4de8-b5d7-4b06b43c6fde", "version": "00.01.000"}], "referenceToPersonOrEntityEnteringTheData": {"shortDescription": [{"value": "Kiwa-Ecobility Experts, Kiwa GmbH (Berlin)", "lang": "en"}], "type": "contact data set", "refObjectId": "eb52a9a8-9d0f-40ce-a5c9-7b78f5615e5a", "version": "00.00.002"}}, "publicationAndOwnership": {"dataSetVersion": "00.00.007", "referenceToRegistrationAuthority": {"shortDescription": [{"value": "Kiwa-Ecobility Experts, Kiwa GmbH (Berlin)", "lang": "en"}], "type": "contact data set", "refObjectId": "eb52a9a8-9d0f-40ce-a5c9-7b78f5615e5a", "version": "00.00.002"}, "registrationNumber": "EPD-Kiwa-EE-193584-EN", "referenceToOwnershipOfDataSet": {"shortDescription": [{"value": "DÖLING Fittings GmbH & Co. KG", "lang": "en"}], "type": "contact data set", "refObjectId": "dcb30f4a-8963-40e4-ab47-6a038a653595", "version": "00.00.001"}, "copyright": true, "licenseType": "Free of charge for all users and uses", "accessRestrictions": [{"value": "None", "lang": "en"}], "other": {"anies": [{"name": "referenceToPublisher", "value": {"shortDescription": [{"value": "Kiwa-Ecobility Experts, Kiwa GmbH (Berlin)", "lang": "en"}], "type": "contact data set", "refObjectId": "eb52a9a8-9d0f-40ce-a5c9-7b78f5615e5a", "version": "00.00.002"}}]}}}, "exchanges": {"exchange": [{"dataSetInternalID": 1, "referenceToFlowDataSet": {"shortDescription": [{"value": "Butt welded Fittings (DÖLING Fittings GmbH & CO KG)", "lang": "en"}], "type": "flow data set", "refObjectId": "448347b8-9da0-4c20-b2d9-a2d47e031b82", "version": "00.00.004"}, "meanAmount": 1.0, "resultingAmount": 1.0, "referenceFlow": true, "resultingflowAmount": 1.0, "flowProperties": [{"name": [{"lang": "en", "value": "Mass"}, {"lang": "de", "value": "Masse"}], "uuid": "93a60a56-a3c8-11da-a746-0800200b9a66", "referenceFlowProperty": true, "meanValue": 1.0, "referenceUnit": "kg", "unitGroupUUID": "ad38d542-3fe9-439d-9b95-2f5f7752acaf"}], "materialProperties": [{"name": "gross density", "value": "7850.0", "unit": "kg/m^3", "unitDescription": "kilograms per cubic metre"}], "typeOfFlow": "Product flow", "classification": {"classHierarchy": "Metalle / Edelstahl / Edelstahl Trinkwasserrohre", "name": "OEKOBAU.DAT"}}, {"dataSetInternalID": 2, "referenceToFlowDataSet": {"shortDescription": [{"value": "Components for re-use (CRU)", "lang": "en"}, {"value": "Komponenten für die Wiederverwendung (CRU)", "lang": "de"}, {"value": "Componentes para su reutilización (CRU)", "lang": "es"}], "type": "flow data set", "refObjectId": "a2b32f97-3fc7-4af2-b209-525bc6426f33", "version": "30.00.000", "uri": "../flows/a2b32f97-3fc7-4af2-b209-525bc6426f33.xml"}, "exchange direction": "OUTPUT", "meanAmount": 0.0, "other": {"anies": [{"value": "0.0", "module": "A1", "scenario": "Standard Scenarios"}, {"value": "0.0", "module": "A2", "scenario": "Standard Scenarios"}, {"value": "0.0", "module": "A3", "scenario": "Standard Scenarios"}, {"value": "0.0", "module": "A1-A3", "scenario": "Standard Scenarios"}, {"value": "0.0", "module": "C1", "scenario": "Standard Scenarios"}, {"value": "0.0", "module": "C2", "scenario": "Standard Scenarios"}, {"value": "0.0", "module": "C3", "scenario": "Standard Scenarios"}, {"value": "0.0", "module": "C4", "scenario": "Standard Scenarios"}, {"value": "0.0", "module": "D", "scenario": "Standard Scenarios"}, {"name": "referenceToUnitGroupDataSet", "value": {"shortDescription": [{"value": "kg", "lang": "en"}], "type": "unit group data set", "refObjectId": "ad38d542-3fe9-439d-9b95-2f5f7752acaf", "version": "30.00.000", "uri": "../unitgroups/ad38d542-3fe9-439d-9b95-2f5f7752acaf.xml"}}]}, "flowProperties": [], "typeOfFlow": "Other flow", "classification": {"classHierarchy": "Größen / Umweltliche Größen / EPD EN 15804 / LCI Indikatoren", "name": "GaBiCategories"}}, {"dataSetInternalID": 3, "referenceToFlowDataSet": {"shortDescription": [{"value": "Exported electrical energy (EEE)", "lang": "en"}, {"value": "Exportierte elektrische Energie (EEE)", "lang": "de"}, {"value": "Energía exportada electrica (EEE)", "lang": "es"}], "type": "flow data set", "refObjectId": "4da0c987-2b76-40d6-9e9e-82a017aaaf29", "version": "30.00.000", "uri": "../flows/4da0c987-2b76-40d6-9e9e-82a017aaaf29.xml"}, "exchange direction": "OUTPUT", "meanAmount": 0.0, "other": {"anies": [{"value": "0.0", "module": "A1", "scenario": "Standard Scenarios"}, {"value": "0.0", "module": "A2", "scenario": "Standard Scenarios"}, {"value": "0.0886763358", "module": "A3", "scenario": "Standard Scenarios"}, {"value": "0.0886763358", "module": "A1-A3", "scenario": "Standard Scenarios"}, {"value": "0.0", "module": "C1", "scenario": "Standard Scenarios"}, {"value": "0.0", "module": "C2", "scenario": "Standard Scenarios"}, {"value": "0.0", "module": "C3", "scenario": "Standard Scenarios"}, {"value": "0.0", "module": "C4", "scenario": "Standard Scenarios"}, {"value": "0.0", "module": "D", "scenario": "Standard Scenarios"}, {"name": "referenceToUnitGroupDataSet", "value": {"shortDescription": [{"value": "MJ", "lang": "en"}], "type": "unit group data set", "refObjectId": "93a60a57-a3c8-11da-a746-0800200c9a66", "version": "03.00.000", "uri": "../unitgroups/93a60a57-a3c8-11da-a746-0800200c9a66.xml"}}]}, "flowProperties": [], "typeOfFlow": "Other flow", "classification": {"classHierarchy": "Größen / Umweltliche Größen / EPD EN 15804 / LCI Indikatoren", "name": "GaBiCategories"}}, {"dataSetInternalID": 4, "referenceToFlowDataSet": {"shortDescription": [{"value": "Exported thermal energy (EET)", "lang": "en"}, {"value": "Exportierte thermische Energie (EET)", "lang": "de"}, {"value": "Energía exportada termal (EET)", "lang": "es"}], "type": "flow data set", "refObjectId": "98daf38a-7a79-46d3-9a37-2b7bd0955810", "version": "30.00.000", "uri": "../flows/98daf38a-7a79-46d3-9a37-2b7bd0955810.xml"}, "exchange direction": "OUTPUT", "meanAmount": 0.0, "other": {"anies": [{"value": "0.0", "module": "A1", "scenario": "Standard Scenarios"}, {"value": "0.0", "module": "A2", "scenario": "Standard Scenarios"}, {"value": "0.1527203561", "module": "A3", "scenario": "Standard Scenarios"}, {"value": "0.1527203561", "module": "A1-A3", "scenario": "Standard Scenarios"}, {"value": "0.0", "module": "C1", "scenario": "Standard Scenarios"}, {"value": "0.0", "module": "C2", "scenario": "Standard Scenarios"}, {"value": "0.0", "module": "C3", "scenario": "Standard Scenarios"}, {"value": "0.0", "module": "C4", "scenario": "Standard Scenarios"}, {"value": "0.0", "module": "D", "scenario": "Standard Scenarios"}, {"name": "referenceToUnitGroupDataSet", "value": {"shortDescription": [{"value": "MJ", "lang": "en"}], "type": "unit group data set", "refObjectId": "93a60a57-a3c8-11da-a746-0800200c9a66", "version": "03.00.000", "uri": "../unitgroups/93a60a57-a3c8-11da-a746-0800200c9a66.xml"}}]}, "flowProperties": [], "typeOfFlow": "Other flow", "classification": {"classHierarchy": "Größen / Umweltliche Größen / EPD EN 15804 / LCI Indikatoren", "name": "GaBiCategories"}}, {"dataSetInternalID": 5, "referenceToFlowDataSet": {"shortDescription": [{"value": "Use of net fresh water (FW)", "lang": "en"}, {"value": "Einsatz von Süßwasserressourcen (FW)", "lang": "de"}, {"value": "Uso neto de recursos de agua dulce (FW)", "lang": "es"}], "type": "flow data set", "refObjectId": "3cf952c8-f3a4-461d-8c96-96456ca62246", "version": "30.00.000", "uri": "../flows/3cf952c8-f3a4-461d-8c96-96456ca62246.xml"}, "exchange direction": "INPUT", "meanAmount": 0.0, "other": {"anies": [{"value": "0.0184", "module": "A1", "scenario": "Standard Scenarios"}, {"value": "1.20032E-4", "module": "A2", "scenario": "Standard Scenarios"}, {"value": "0.00122512779467", "module": "A3", "scenario": "Standard Scenarios"}, {"value": "0.019745159794669998", "module": "A1-A3", "scenario": "Standard Scenarios"}, {"value": "0.0", "module": "C1", "scenario": "Standard Scenarios"}, {"value": "7.44E-7", "module": "C2", "scenario": "Standard Scenarios"}, {"value": "0.0", "module": "C3", "scenario": "Standard Scenarios"}, {"value": "1.509438137E-4", "module": "C4", "scenario": "Standard Scenarios"}, {"value": "-2.060304418E-4", "module": "D", "scenario": "Standard Scenarios"}, {"name": "referenceToUnitGroupDataSet", "value": {"shortDescription": [{"value": "m3", "lang": "en"}], "type": "unit group data set", "refObjectId": "cd950537-0a98-4044-9ba7-9f9a68d0a504", "version": "30.00.000", "uri": "../unitgroups/cd950537-0a98-4044-9ba7-9f9a68d0a504.xml"}}]}, "flowProperties": [], "typeOfFlow": "Other flow", "classification": {"classHierarchy": "Größen / Umweltliche Größen / EPD EN 15804 / LCI Indikatoren", "name": "GaBiCategories"}}, {"dataSetInternalID": 6, "referenceToFlowDataSet": {"shortDescription": [{"value": "Hazardous waste disposed (HWD)", "lang": "en"}, {"value": "Gefährlicher Abfall zur Deponie (HWD)", "lang": "de"}, {"value": "Residuos peligrosos eliminados (HWD)", "lang": "es"}], "type": "flow data set", "refObjectId": "430f9e0f-59b2-46a0-8e0d-55e0e84948fc", "version": "30.00.000", "uri": "../flows/430f9e0f-59b2-46a0-8e0d-55e0e84948fc.xml"}, "exchange direction": "OUTPUT", "meanAmount": 0.0, "other": {"anies": [{"value": "0.0117", "module": "A1", "scenario": "Standard Scenarios"}, {"value": "2.49744E-6", "module": "A2", "scenario": "Standard Scenarios"}, {"value": "0.01452788743816", "module": "A3", "scenario": "Standard Scenarios"}, {"value": "0.02623038487816", "module": "A1-A3", "scenario": "Standard Scenarios"}, {"value": "0.0", "module": "C1", "scenario": "Standard Scenarios"}, {"value": "1.548E-8", "module": "C2", "scenario": "Standard Scenarios"}, {"value": "0.0", "module": "C3", "scenario": "Standard Scenarios"}, {"value": "2.1118991E-7", "module": "C4", "scenario": "Standard Scenarios"}, {"value": "-6.83175674E-6", "module": "D", "scenario": "Standard Scenarios"}, {"name": "referenceToUnitGroupDataSet", "value": {"shortDescription": [{"value": "kg", "lang": "en"}], "type": "unit group data set", "refObjectId": "ad38d542-3fe9-439d-9b95-2f5f7752acaf", "version": "30.00.000", "uri": "../unitgroups/ad38d542-3fe9-439d-9b95-2f5f7752acaf.xml"}}]}, "flowProperties": [], "typeOfFlow": "Other flow", "classification": {"classHierarchy": "Größen / Umweltliche Größen / EPD EN 15804 / LCI Indikatoren", "name": "GaBiCategories"}}, {"dataSetInternalID": 7, "referenceToFlowDataSet": {"shortDescription": [{"value": "Materials for energy recovery (MER)", "lang": "en"}, {"value": "Stoffe für die Energierückgewinnung (MER)", "lang": "de"}, {"value": "Materiales para valorización energética (recuperación de energía) (MER)", "lang": "es"}], "type": "flow data set", "refObjectId": "59a9181c-3aaf-46ee-8b13-2b3723b6e447", "version": "30.00.000", "uri": "../flows/59a9181c-3aaf-46ee-8b13-2b3723b6e447.xml"}, "exchange direction": "OUTPUT", "meanAmount": 0.0, "other": {"anies": [{"value": "0.0", "module": "A1", "scenario": "Standard Scenarios"}, {"value": "0.0", "module": "A2", "scenario": "Standard Scenarios"}, {"value": "0.0", "module": "A3", "scenario": "Standard Scenarios"}, {"value": "0.0", "module": "A1-A3", "scenario": "Standard Scenarios"}, {"value": "0.0", "module": "C1", "scenario": "Standard Scenarios"}, {"value": "0.0", "module": "C2", "scenario": "Standard Scenarios"}, {"value": "0.0", "module": "C3", "scenario": "Standard Scenarios"}, {"value": "0.0", "module": "C4", "scenario": "Standard Scenarios"}, {"value": "0.0", "module": "D", "scenario": "Standard Scenarios"}, {"name": "referenceToUnitGroupDataSet", "value": {"shortDescription": [{"value": "kg", "lang": "en"}], "type": "unit group data set", "refObjectId": "ad38d542-3fe9-439d-9b95-2f5f7752acaf", "version": "30.00.000", "uri": "../unitgroups/ad38d542-3fe9-439d-9b95-2f5f7752acaf.xml"}}]}, "flowProperties": [], "typeOfFlow": "Other flow", "classification": {"classHierarchy": "Größen / Umweltliche Größen / EPD EN 15804 / LCI Indikatoren", "name": "GaBiCategories"}}, {"dataSetInternalID": 8, "referenceToFlowDataSet": {"shortDescription": [{"value": "Materials for recycling (MFR)", "lang": "en"}, {"value": "Stoffe zum Recycling (MFR)", "lang": "de"}, {"value": "Materiales para el reciclaje (MFR)", "lang": "es"}], "type": "flow data set", "refObjectId": "d7fe48a5-4103-49c8-9aae-b0b5dfdbd6ae", "version": "30.00.000", "uri": "../flows/d7fe48a5-4103-49c8-9aae-b0b5dfdbd6ae.xml"}, "exchange direction": "OUTPUT", "meanAmount": 0.0, "other": {"anies": [{"value": "0.216", "module": "A1", "scenario": "Standard Scenarios"}, {"value": "0.0", "module": "A2", "scenario": "Standard Scenarios"}, {"value": "0.007168", "module": "A3", "scenario": "Standard Scenarios"}, {"value": "0.223168", "module": "A1-A3", "scenario": "Standard Scenarios"}, {"value": "0.0", "module": "C1", "scenario": "Standard Scenarios"}, {"value": "0.0", "module": "C2", "scenario": "Standard Scenarios"}, {"value": "0.04", "module": "C3", "scenario": "Standard Scenarios"}, {"value": "0.0", "module": "C4", "scenario": "Standard Scenarios"}, {"value": "0.0", "module": "D", "scenario": "Standard Scenarios"}, {"name": "referenceToUnitGroupDataSet", "value": {"shortDescription": [{"value": "kg", "lang": "en"}], "type": "unit group data set", "refObjectId": "ad38d542-3fe9-439d-9b95-2f5f7752acaf", "version": "30.00.000", "uri": "../unitgroups/ad38d542-3fe9-439d-9b95-2f5f7752acaf.xml"}}]}, "flowProperties": [], "typeOfFlow": "Other flow", "classification": {"classHierarchy": "Größen / Umweltliche Größen / EPD EN 15804 / LCI Indikatoren", "name": "GaBiCategories"}}, {"dataSetInternalID": 9, "referenceToFlowDataSet": {"shortDescription": [{"value": "Non-hazardous waste disposed (NHWD)", "lang": "en"}, {"value": "Entsorgter nicht gefährlicher Abfall (NHWD)", "lang": "de"}, {"value": "Residuos no peligrosos eliminados (NHWD)", "lang": "es"}], "type": "flow data set", "refObjectId": "b29ef66b-e286-4afa-949f-62f1a7b4d7fa", "version": "30.00.000", "uri": "../flows/b29ef66b-e286-4afa-949f-62f1a7b4d7fa.xml"}, "exchange direction": "OUTPUT", "meanAmount": 0.0, "other": {"anies": [{"value": "0.00742", "module": "A1", "scenario": "Standard Scenarios"}, {"value": "0.06248924", "module": "A2", "scenario": "Standard Scenarios"}, {"value": "0.03566410942067", "module": "A3", "scenario": "Standard Scenarios"}, {"value": "0.10557334942067", "module": "A1-A3", "scenario": "Standard Scenarios"}, {"value": "0.0", "module": "C1", "scenario": "Standard Scenarios"}, {"value": "3.8733E-4", "module": "C2", "scenario": "Standard Scenarios"}, {"value": "0.0", "module": "C3", "scenario": "Standard Scenarios"}, {"value": "0.95970682967145", "module": "C4", "scenario": "Standard Scenarios"}, {"value": "-0.00557741139614", "module": "D", "scenario": "Standard Scenarios"}, {"name": "referenceToUnitGroupDataSet", "value": {"shortDescription": [{"value": "kg", "lang": "en"}], "type": "unit group data set", "refObjectId": "ad38d542-3fe9-439d-9b95-2f5f7752acaf", "version": "30.00.000", "uri": "../unitgroups/ad38d542-3fe9-439d-9b95-2f5f7752acaf.xml"}}]}, "flowProperties": [], "typeOfFlow": "Other flow", "classification": {"classHierarchy": "Größen / Umweltliche Größen / EPD EN 15804 / LCI Indikatoren", "name": "GaBiCategories"}}, {"dataSetInternalID": 10, "referenceToFlowDataSet": {"shortDescription": [{"value": "Use of non renewable secondary fuels (NRSF)", "lang": "en"}, {"value": "Nicht erneuerbare Sekundärbrennstoffe (NRSF)", "lang": "de"}, {"value": "Uso de combustibles secundarios no renovables (NRSF)", "lang": "es"}], "type": "flow data set", "refObjectId": "89def144-d39a-4287-b86f-efde453ddcb2", "version": "30.00.000", "uri": "../flows/89def144-d39a-4287-b86f-efde453ddcb2.xml"}, "exchange direction": "INPUT", "meanAmount": 0.0, "other": {"anies": [{"value": "0.0", "module": "A1", "scenario": "Standard Scenarios"}, {"value": "0.0", "module": "A2", "scenario": "Standard Scenarios"}, {"value": "0.0", "module": "A3", "scenario": "Standard Scenarios"}, {"value": "0.0", "module": "A1-A3", "scenario": "Standard Scenarios"}, {"value": "0.0", "module": "C1", "scenario": "Standard Scenarios"}, {"value": "0.0", "module": "C2", "scenario": "Standard Scenarios"}, {"value": "0.0", "module": "C3", "scenario": "Standard Scenarios"}, {"value": "0.0", "module": "C4", "scenario": "Standard Scenarios"}, {"value": "0.0", "module": "D", "scenario": "Standard Scenarios"}, {"name": "referenceToUnitGroupDataSet", "value": {"shortDescription": [{"value": "MJ", "lang": "en"}], "type": "unit group data set", "refObjectId": "93a60a57-a3c8-11da-a746-0800200c9a66", "version": "03.00.000", "uri": "../unitgroups/93a60a57-a3c8-11da-a746-0800200c9a66.xml"}}]}, "flowProperties": [], "typeOfFlow": "Other flow", "classification": {"classHierarchy": "Größen / Umweltliche Größen / EPD EN 15804 / LCI Indikatoren", "name": "GaBiCategories"}}, {"dataSetInternalID": 11, "referenceToFlowDataSet": {"shortDescription": [{"value": "Use of non renewable primary energy (PENRE)", "lang": "en"}, {"value": "Nicht-erneuerbare Primärenergie als Energieträger (PENRE)", "lang": "de"}, {"value": "Uso de energía primaria no renovable, excluyendo los recursos de energía primaria no renovable utilizada como materia prima (PENRE)", "lang": "es"}], "type": "flow data set", "refObjectId": "ac857178-2b45-46ec-892a-a9a4332f0372", "version": "38.00.000", "uri": "../flows/ac857178-2b45-46ec-892a-a9a4332f0372.xml"}, "exchange direction": "INPUT", "meanAmount": 0.0, "other": {"anies": [{"value": "35.2", "module": "A1", "scenario": "Standard Scenarios"}, {"value": "1.04592642", "module": "A2", "scenario": "Standard Scenarios"}, {"value": "2.40600266954794", "module": "A3", "scenario": "Standard Scenarios"}, {"value": "38.65192908954794", "module": "A1-A3", "scenario": "Standard Scenarios"}, {"value": "0.0", "module": "C1", "scenario": "Standard Scenarios"}, {"value": "0.006483015", "module": "C2", "scenario": "Standard Scenarios"}, {"value": "0.0", "module": "C3", "scenario": "Standard Scenarios"}, {"value": "0.15012064091365", "module": "C4", "scenario": "Standard Scenarios"}, {"value": "-0.41291069739726", "module": "D", "scenario": "Standard Scenarios"}, {"name": "referenceToUnitGroupDataSet", "value": {"shortDescription": [{"value": "MJ", "lang": "en"}], "type": "unit group data set", "refObjectId": "93a60a57-a3c8-11da-a746-0800200c9a66", "version": "03.00.000", "uri": "../unitgroups/93a60a57-a3c8-11da-a746-0800200c9a66.xml"}}]}, "flowProperties": [], "typeOfFlow": "Other flow", "classification": {"classHierarchy": "Quantities", "name": "GaBiCategories"}}, {"dataSetInternalID": 12, "referenceToFlowDataSet": {"shortDescription": [{"value": "Use of non renewable primary energy resources used as raw materials (PENRM)", "lang": "en"}, {"value": "Nicht-erneuerbare Primärenergie zur stofflichen Nutzung (PENRM)", "lang": "de"}, {"value": "Uso de la energía primaria no renovable utilizada como materia prima (PENRM)", "lang": "es"}], "type": "flow data set", "refObjectId": "1421caa0-679d-4bf4-b282-0eb850ccae27", "version": "38.00.000", "uri": "../flows/1421caa0-679d-4bf4-b282-0eb850ccae27.xml"}, "exchange direction": "INPUT", "meanAmount": 0.0, "other": {"anies": [{"value": "0.00624", "module": "A1", "scenario": "Standard Scenarios"}, {"value": "0.0", "module": "A2", "scenario": "Standard Scenarios"}, {"value": "0.49282103", "module": "A3", "scenario": "Standard Scenarios"}, {"value": "0.49906103", "module": "A1-A3", "scenario": "Standard Scenarios"}, {"value": "0.0", "module": "C1", "scenario": "Standard Scenarios"}, {"value": "0.0", "module": "C2", "scenario": "Standard Scenarios"}, {"value": "0.0", "module": "C3", "scenario": "Standard Scenarios"}, {"value": "0.0", "module": "C4", "scenario": "Standard Scenarios"}, {"value": "0.0", "module": "D", "scenario": "Standard Scenarios"}, {"name": "referenceToUnitGroupDataSet", "value": {"shortDescription": [{"value": "MJ", "lang": "en"}], "type": "unit group data set", "refObjectId": "93a60a57-a3c8-11da-a746-0800200c9a66", "version": "03.00.000", "uri": "../unitgroups/93a60a57-a3c8-11da-a746-0800200c9a66.xml"}}]}, "flowProperties": [], "typeOfFlow": "Other flow", "classification": {"classHierarchy": "Quantities", "name": "GaBiCategories"}}, {"dataSetInternalID": 13, "referenceToFlowDataSet": {"shortDescription": [{"value": "Total use of non-renewable primary energy resources (PENRT)", "lang": "en"}, {"value": "Total nicht erneuerbare Primärenergie (PENRT)", "lang": "de"}, {"value": "Uso total de la energía primaria no renovable (energía primaria y recursos de energía primaria renovable utilizada como materia prima) (PENRT)", "lang": "es"}], "type": "flow data set", "refObjectId": "06159210-646b-4c8d-8583-da9b3b95a6c1", "version": "30.00.000", "uri": "../flows/06159210-646b-4c8d-8583-da9b3b95a6c1.xml"}, "exchange direction": "INPUT", "meanAmount": 0.0, "other": {"anies": [{"value": "35.20624", "module": "A1", "scenario": "Standard Scenarios"}, {"value": "1.04592642", "module": "A2", "scenario": "Standard Scenarios"}, {"value": "2.89882369954794", "module": "A3", "scenario": "Standard Scenarios"}, {"value": "39.15099011954794", "module": "A1-A3", "scenario": "Standard Scenarios"}, {"value": "0.0", "module": "C1", "scenario": "Standard Scenarios"}, {"value": "0.006483015", "module": "C2", "scenario": "Standard Scenarios"}, {"value": "0.0", "module": "C3", "scenario": "Standard Scenarios"}, {"value": "0.15012064091365", "module": "C4", "scenario": "Standard Scenarios"}, {"value": "-0.41291069739726", "module": "D", "scenario": "Standard Scenarios"}, {"name": "referenceToUnitGroupDataSet", "value": {"shortDescription": [{"value": "MJ", "lang": "en"}], "type": "unit group data set", "refObjectId": "93a60a57-a3c8-11da-a746-0800200c9a66", "version": "03.00.000", "uri": "../unitgroups/93a60a57-a3c8-11da-a746-0800200c9a66.xml"}}]}, "flowProperties": [], "typeOfFlow": "Other flow", "classification": {"classHierarchy": "Größen / Umweltliche Größen / EPD EN 15804 / LCI Indikatoren", "name": "GaBiCategories"}}, {"dataSetInternalID": 14, "referenceToFlowDataSet": {"shortDescription": [{"value": "Use of renewable primary energy (PERE)", "lang": "en"}, {"value": "Erneuerbare Primärenergie als Energieträger (PERE)", "lang": "de"}, {"value": "Uso de energía primaria renovable excluyendo los recursos de energía primaria renovable utilizada como materia prima (PERE)", "lang": "es"}], "type": "flow data set", "refObjectId": "20f32be5-0398-4288-9b6d-accddd195317", "version": "38.00.000", "uri": "../flows/20f32be5-0398-4288-9b6d-accddd195317.xml"}, "exchange direction": "INPUT", "meanAmount": 0.0, "other": {"anies": [{"value": "0.703", "module": "A1", "scenario": "Standard Scenarios"}, {"value": "0.012332804", "module": "A2", "scenario": "Standard Scenarios"}, {"value": "0.0744174800275", "module": "A3", "scenario": "Standard Scenarios"}, {"value": "0.7897502840275", "module": "A1-A3", "scenario": "Standard Scenarios"}, {"value": "0.0", "module": "C1", "scenario": "Standard Scenarios"}, {"value": "7.6443E-5", "module": "C2", "scenario": "Standard Scenarios"}, {"value": "0.0", "module": "C3", "scenario": "Standard Scenarios"}, {"value": "0.00114269416765", "module": "C4", "scenario": "Standard Scenarios"}, {"value": "0.01156001979275", "module": "D", "scenario": "Standard Scenarios"}, {"name": "referenceToUnitGroupDataSet", "value": {"shortDescription": [{"value": "MJ", "lang": "en"}], "type": "unit group data set", "refObjectId": "93a60a57-a3c8-11da-a746-0800200c9a66", "version": "03.00.000", "uri": "../unitgroups/93a60a57-a3c8-11da-a746-0800200c9a66.xml"}}]}, "flowProperties": [], "typeOfFlow": "Other flow", "classification": {"classHierarchy": "Quantities", "name": "GaBiCategories"}}, {"dataSetInternalID": 15, "referenceToFlowDataSet": {"shortDescription": [{"value": "Use of renewable primary energy resources used as raw materials (PERM)", "lang": "en"}, {"value": "Erneuerbare Primärenergie zur stofflichen Nutzung (PERM)", "lang": "de"}, {"value": "Uso de energía primaria renovable utilizada como materia prima (PERM)", "lang": "es"}], "type": "flow data set", "refObjectId": "fb3ec0de-548d-4508-aea5-00b73bf6f702", "version": "38.00.000", "uri": "../flows/fb3ec0de-548d-4508-aea5-00b73bf6f702.xml"}, "exchange direction": "INPUT", "meanAmount": 0.0, "other": {"anies": [{"value": "0.0", "module": "A1", "scenario": "Standard Scenarios"}, {"value": "0.0", "module": "A2", "scenario": "Standard Scenarios"}, {"value": "0.0063664293", "module": "A3", "scenario": "Standard Scenarios"}, {"value": "0.0063664293", "module": "A1-A3", "scenario": "Standard Scenarios"}, {"value": "0.0", "module": "C1", "scenario": "Standard Scenarios"}, {"value": "0.0", "module": "C2", "scenario": "Standard Scenarios"}, {"value": "0.0", "module": "C3", "scenario": "Standard Scenarios"}, {"value": "0.0", "module": "C4", "scenario": "Standard Scenarios"}, {"value": "0.0", "module": "D", "scenario": "Standard Scenarios"}, {"name": "referenceToUnitGroupDataSet", "value": {"shortDescription": [{"value": "MJ", "lang": "en"}], "type": "unit group data set", "refObjectId": "93a60a57-a3c8-11da-a746-0800200c9a66", "version": "03.00.000", "uri": "../unitgroups/93a60a57-a3c8-11da-a746-0800200c9a66.xml"}}]}, "flowProperties": [], "typeOfFlow": "Other flow", "classification": {"classHierarchy": "Quantities", "name": "GaBiCategories"}}, {"dataSetInternalID": 16, "referenceToFlowDataSet": {"shortDescription": [{"value": "Total use of renewable primary energy resources (PERT)", "lang": "en"}, {"value": "Total erneuerbare Primärenergie (PERT)", "lang": "de"}, {"value": "Uso total de la energía primaria renovable (energía primaria y recursos de energía primaria renovable utilizada como materia prima) (PERT)", "lang": "es"}], "type": "flow data set", "refObjectId": "53f97275-fa8a-4cdd-9024-65936002acd0", "version": "30.00.000", "uri": "../flows/53f97275-fa8a-4cdd-9024-65936002acd0.xml"}, "exchange direction": "INPUT", "meanAmount": 0.0, "other": {"anies": [{"value": "0.703", "module": "A1", "scenario": "Standard Scenarios"}, {"value": "0.012332804", "module": "A2", "scenario": "Standard Scenarios"}, {"value": "0.0807839093275", "module": "A3", "scenario": "Standard Scenarios"}, {"value": "0.7961167133275", "module": "A1-A3", "scenario": "Standard Scenarios"}, {"value": "0.0", "module": "C1", "scenario": "Standard Scenarios"}, {"value": "7.6443E-5", "module": "C2", "scenario": "Standard Scenarios"}, {"value": "0.0", "module": "C3", "scenario": "Standard Scenarios"}, {"value": "0.00114269416765", "module": "C4", "scenario": "Standard Scenarios"}, {"value": "0.01156001979275", "module": "D", "scenario": "Standard Scenarios"}, {"name": "referenceToUnitGroupDataSet", "value": {"shortDescription": [{"value": "MJ", "lang": "en"}], "type": "unit group data set", "refObjectId": "93a60a57-a3c8-11da-a746-0800200c9a66", "version": "03.00.000", "uri": "../unitgroups/93a60a57-a3c8-11da-a746-0800200c9a66.xml"}}]}, "flowProperties": [], "typeOfFlow": "Other flow", "classification": {"classHierarchy": "Größen / Umweltliche Größen / EPD EN 15804 / LCI Indikatoren", "name": "GaBiCategories"}}, {"dataSetInternalID": 17, "referenceToFlowDataSet": {"shortDescription": [{"value": "Use of renewable secondary fuels (RSF)", "lang": "en"}, {"value": "Erneuerbare Sekundärbrennstoffe (RSF)", "lang": "de"}, {"value": "Uso de combustibles secundarios renovables (RSF)", "lang": "es"}], "type": "flow data set", "refObjectId": "64333088-a55f-4aa2-9a31-c10b07816787", "version": "30.00.000", "uri": "../flows/64333088-a55f-4aa2-9a31-c10b07816787.xml"}, "exchange direction": "INPUT", "meanAmount": 0.0, "other": {"anies": [{"value": "0.0", "module": "A1", "scenario": "Standard Scenarios"}, {"value": "0.0", "module": "A2", "scenario": "Standard Scenarios"}, {"value": "0.0", "module": "A3", "scenario": "Standard Scenarios"}, {"value": "0.0", "module": "A1-A3", "scenario": "Standard Scenarios"}, {"value": "0.0", "module": "C1", "scenario": "Standard Scenarios"}, {"value": "0.0", "module": "C2", "scenario": "Standard Scenarios"}, {"value": "0.0", "module": "C3", "scenario": "Standard Scenarios"}, {"value": "0.0", "module": "C4", "scenario": "Standard Scenarios"}, {"value": "0.0", "module": "D", "scenario": "Standard Scenarios"}, {"name": "referenceToUnitGroupDataSet", "value": {"shortDescription": [{"value": "MJ", "lang": "en"}], "type": "unit group data set", "refObjectId": "93a60a57-a3c8-11da-a746-0800200c9a66", "version": "03.00.000", "uri": "../unitgroups/93a60a57-a3c8-11da-a746-0800200c9a66.xml"}}]}, "flowProperties": [], "typeOfFlow": "Other flow", "classification": {"classHierarchy": "Größen / Umweltliche Größen / EPD EN 15804 / LCI Indikatoren", "name": "GaBiCategories"}}, {"dataSetInternalID": 18, "referenceToFlowDataSet": {"shortDescription": [{"value": "Radioactive waste disposed (RWD)", "lang": "en"}, {"value": "Entsorgter radioaktiver Abfall (RWD)", "lang": "de"}, {"value": "Residuos radiactivos eliminados (RWD)", "lang": "es"}], "type": "flow data set", "refObjectId": "3449546e-52ad-4b39-b809-9fb77cea8ff6", "version": "30.00.000", "uri": "../flows/3449546e-52ad-4b39-b809-9fb77cea8ff6.xml"}, "exchange direction": "OUTPUT", "meanAmount": 0.0, "other": {"anies": [{"value": "0.0", "module": "A1", "scenario": "Standard Scenarios"}, {"value": "6.4856E-6", "module": "A2", "scenario": "Standard Scenarios"}, {"value": "8.40093144E-6", "module": "A3", "scenario": "Standard Scenarios"}, {"value": "1.4886531440000001E-5", "module": "A1-A3", "scenario": "Standard Scenarios"}, {"value": "0.0", "module": "C1", "scenario": "Standard Scenarios"}, {"value": "4.02E-8", "module": "C2", "scenario": "Standard Scenarios"}, {"value": "0.0", "module": "C3", "scenario": "Standard Scenarios"}, {"value": "9.2813297E-7", "module": "C4", "scenario": "Standard Scenarios"}, {"value": "3.3708342E-7", "module": "D", "scenario": "Standard Scenarios"}, {"name": "referenceToUnitGroupDataSet", "value": {"shortDescription": [{"value": "kg", "lang": "en"}], "type": "unit group data set", "refObjectId": "ad38d542-3fe9-439d-9b95-2f5f7752acaf", "version": "30.00.000", "uri": "../unitgroups/ad38d542-3fe9-439d-9b95-2f5f7752acaf.xml"}}]}, "flowProperties": [], "typeOfFlow": "Other flow", "classification": {"classHierarchy": "Größen / Umweltliche Größen / EPD EN 15804 / LCI Indikatoren", "name": "GaBiCategories"}}, {"dataSetInternalID": 19, "referenceToFlowDataSet": {"shortDescription": [{"value": "Use of secondary material (SM)", "lang": "en"}, {"value": "Einsatz von Sekundärstoffen (SM)", "lang": "de"}, {"value": "Uso de materiales secundarios (SM)", "lang": "es"}], "type": "flow data set", "refObjectId": "c6a1f35f-2d09-4f54-8dfb-97e502e1ce92", "version": "30.00.000", "uri": "../flows/c6a1f35f-2d09-4f54-8dfb-97e502e1ce92.xml"}, "exchange direction": "INPUT", "meanAmount": 0.0, "other": {"anies": [{"value": "1.21", "module": "A1", "scenario": "Standard Scenarios"}, {"value": "0.0", "module": "A2", "scenario": "Standard Scenarios"}, {"value": "0.03756193", "module": "A3", "scenario": "Standard Scenarios"}, {"value": "1.24756193", "module": "A1-A3", "scenario": "Standard Scenarios"}, {"value": "0.0", "module": "C1", "scenario": "Standard Scenarios"}, {"value": "0.0", "module": "C2", "scenario": "Standard Scenarios"}, {"value": "0.0", "module": "C3", "scenario": "Standard Scenarios"}, {"value": "0.0", "module": "C4", "scenario": "Standard Scenarios"}, {"value": "0.0", "module": "D", "scenario": "Standard Scenarios"}, {"name": "referenceToUnitGroupDataSet", "value": {"shortDescription": [{"value": "kg", "lang": "en"}], "type": "unit group data set", "refObjectId": "ad38d542-3fe9-439d-9b95-2f5f7752acaf", "version": "30.00.000", "uri": "../unitgroups/ad38d542-3fe9-439d-9b95-2f5f7752acaf.xml"}}]}, "flowProperties": [], "typeOfFlow": "Other flow", "classification": {"classHierarchy": "Größen / Umweltliche Größen / EPD EN 15804 / LCI Indikatoren", "name": "GaBiCategories"}}]}, "LCIAResults": {"LCIAResult": [{"referenceToLCIAMethodDataSet": {"shortDescription": [{"value": "Abiotic depletion potential - non-fossil resources (ADPE)", "lang": "en"}, {"value": "Potenzial für die Verknappung abiotischer Ressourcen – nicht fossile Ressourcen (ADPE)", "lang": "de"}], "type": "LCIA method data set", "refObjectId": "b2ad6494-c78d-11e6-9d9d-cec0c932ce01", "version": "01.00.011", "uri": "../lciamethods/b2ad6494-c78d-11e6-9d9d-cec0c932ce01.xml"}, "meanAmount": 0.0, "other": {"anies": [{"value": "5.32E-5", "module": "A1", "scenario": "Standard Scenarios"}, {"value": "1.65528E-6", "module": "A2", "scenario": "Standard Scenarios"}, {"value": "3.29252767E-6", "module": "A3", "scenario": "Standard Scenarios"}, {"value": "5.8147807670000003E-5", "module": "A1-A3", "scenario": "Standard Scenarios"}, {"value": "0.0", "module": "C1", "scenario": "Standard Scenarios"}, {"value": "1.026E-8", "module": "C2", "scenario": "Standard Scenarios"}, {"value": "0.0", "module": "C3", "scenario": "Standard Scenarios"}, {"value": "4.626301E-8", "module": "C4", "scenario": "Standard Scenarios"}, {"value": "-3.848416E-8", "module": "D", "scenario": "Standard Scenarios"}, {"name": "referenceToUnitGroupDataSet", "value": {"shortDescription": [{"value": "kg Sb-eq.", "lang": "en"}], "type": "unit group data set", "refObjectId": "54ccd2d9-a32a-4fc2-923d-f2c8c93e89d4", "version": "30.00.000", "uri": "../unitgroups/54ccd2d9-a32a-4fc2-923d-f2c8c93e89d4.xml"}}]}}, {"referenceToLCIAMethodDataSet": {"shortDescription": [{"value": "Abiotic depletion potential - fossil resources (ADPF)", "lang": "en"}, {"value": "Potenzial für die Verknappung abiotischer Ressourcen – fossile Brennstoffe (ADPF)", "lang": "de"}], "type": "LCIA method data set", "refObjectId": "b2ad6110-c78d-11e6-9d9d-cec0c932ce01", "version": "01.00.011", "uri": "../lciamethods/b2ad6110-c78d-11e6-9d9d-cec0c932ce01.xml"}, "meanAmount": 0.0, "other": {"anies": [{"value": "31.6", "module": "A1", "scenario": "Standard Scenarios"}, {"value": "0.985120532", "module": "A2", "scenario": "Standard Scenarios"}, {"value": "2.71581056663579", "module": "A3", "scenario": "Standard Scenarios"}, {"value": "35.30093109863579", "module": "A1-A3", "scenario": "Standard Scenarios"}, {"value": "0.0", "module": "C1", "scenario": "Standard Scenarios"}, {"value": "0.006106119", "module": "C2", "scenario": "Standard Scenarios"}, {"value": "0.0", "module": "C3", "scenario": "Standard Scenarios"}, {"value": "0.14132853572812", "module": "C4", "scenario": "Standard Scenarios"}, {"value": "-0.39785084399246", "module": "D", "scenario": "Standard Scenarios"}, {"name": "referenceToUnitGroupDataSet", "value": {"shortDescription": [{"value": "MJ", "lang": "en"}], "type": "unit group data set", "refObjectId": "93a60a57-a3c8-11da-a746-0800200c9a66", "version": "03.00.000", "uri": "../unitgroups/93a60a57-a3c8-11da-a746-0800200c9a66.xml"}}]}}, {"referenceToLCIAMethodDataSet": {"shortDescription": [{"value": "Acidification potential, Accumulated Exceedance (AP)", "lang": "en"}, {"value": "Versauerungspotenzial, kumulierte Überschreitung (AP)", "lang": "de"}], "type": "LCIA method data set", "refObjectId": "b5c611c6-def3-11e6-bf01-fe55135034f3", "version": "01.03.010", "uri": "../lciamethods/b5c611c6-def3-11e6-bf01-fe55135034f3.xml"}, "meanAmount": 0.0, "other": {"anies": [{"value": "0.00612", "module": "A1", "scenario": "Standard Scenarios"}, {"value": "3.78972E-4", "module": "A2", "scenario": "Standard Scenarios"}, {"value": "4.7145202616E-4", "module": "A3", "scenario": "Standard Scenarios"}, {"value": "0.00697042402616", "module": "A1-A3", "scenario": "Standard Scenarios"}, {"value": "0.0", "module": "C1", "scenario": "Standard Scenarios"}, {"value": "2.349E-6", "module": "C2", "scenario": "Standard Scenarios"}, {"value": "0.0", "module": "C3", "scenario": "Standard Scenarios"}, {"value": "4.799104832E-5", "module": "C4", "scenario": "Standard Scenarios"}, {"value": "-2.1984991456E-4", "module": "D", "scenario": "Standard Scenarios"}, {"name": "referenceToUnitGroupDataSet", "value": {"shortDescription": [{"value": "mol H+-eq.", "lang": "en"}], "type": "unit group data set", "refObjectId": "42e089ac-92bf-4bf2-8ca1-5fc40d18f2ed", "version": "00.01.000", "uri": "../unitgroups/42e089ac-92bf-4bf2-8ca1-5fc40d18f2ed.xml"}}]}}, {"referenceToLCIAMethodDataSet": {"shortDescription": [{"value": "Eutrophication potential - freshwater (EP-freshwater)", "lang": "en"}, {"value": "Eutrophierungspotenzial - Süßwasser (EP-freshwater)", "lang": "de"}], "type": "LCIA method data set", "refObjectId": "b53ec18f-7377-4ad3-86eb-cc3f4f276b2b", "version": "01.00.011", "uri": "../lciamethods/b53ec18f-7377-4ad3-86eb-cc3f4f276b2b.xml"}, "meanAmount": 0.0, "other": {"anies": [{"value": "2.55E-5", "module": "A1", "scenario": "Standard Scenarios"}, {"value": "6.5824E-7", "module": "A2", "scenario": "Standard Scenarios"}, {"value": "4.19284899E-6", "module": "A3", "scenario": "Standard Scenarios"}, {"value": "3.0351088989999998E-5", "module": "A1-A3", "scenario": "Standard Scenarios"}, {"value": "0.0", "module": "C1", "scenario": "Standard Scenarios"}, {"value": "4.08E-9", "module": "C2", "scenario": "Standard Scenarios"}, {"value": "0.0", "module": "C3", "scenario": "Standard Scenarios"}, {"value": "5.666221E-8", "module": "C4", "scenario": "Standard Scenarios"}, {"value": "-2.01118046E-6", "module": "D", "scenario": "Standard Scenarios"}, {"name": "referenceToUnitGroupDataSet", "value": {"shortDescription": [{"value": "kg P-eq.", "lang": "en"}], "type": "unit group data set", "refObjectId": "0429039d-a61d-4590-ba67-aa4a20a810a1", "version": "30.00.000", "uri": "../unitgroups/0429039d-a61d-4590-ba67-aa4a20a810a1.xml"}}]}}, {"referenceToLCIAMethodDataSet": {"shortDescription": [{"value": "Eutrophication potential - marine (EP-marine)", "lang": "en"}, {"value": "Eutrophierungspotenzial - Salzwasser (EP-marine)", "lang": "de"}], "type": "LCIA method data set", "refObjectId": "b5c619fa-def3-11e6-bf01-fe55135034f3", "version": "02.00.011", "uri": "../lciamethods/b5c619fa-def3-11e6-bf01-fe55135034f3.xml"}, "meanAmount": 0.0, "other": {"anies": [{"value": "0.00124", "module": "A1", "scenario": "Standard Scenarios"}, {"value": "1.33584E-4", "module": "A2", "scenario": "Standard Scenarios"}, {"value": "9.002752775E-5", "module": "A3", "scenario": "Standard Scenarios"}, {"value": "0.00146361152775", "module": "A1-A3", "scenario": "Standard Scenarios"}, {"value": "0.0", "module": "C1", "scenario": "Standard Scenarios"}, {"value": "8.28E-7", "module": "C2", "scenario": "Standard Scenarios"}, {"value": "0.0", "module": "C3", "scenario": "Standard Scenarios"}, {"value": "1.650484258E-5", "module": "C4", "scenario": "Standard Scenarios"}, {"value": "-4.077274891E-5", "module": "D", "scenario": "Standard Scenarios"}, {"name": "referenceToUnitGroupDataSet", "value": {"shortDescription": [{"value": "kg N-eq.", "lang": "en"}], "type": "unit group data set", "refObjectId": "d05bb823-ecdf-4686-8c40-bf1d9257859f", "version": "00.00.003", "uri": "../unitgroups/d05bb823-ecdf-4686-8c40-bf1d9257859f.xml"}}]}}, {"referenceToLCIAMethodDataSet": {"shortDescription": [{"value": "Eutrophication potential - terrestrial (EP-terrestrial)", "lang": "en"}, {"value": "Eutrophierungspotenzial - Land (EP-terrestrial)", "lang": "de"}], "type": "LCIA method data set", "refObjectId": "b5c614d2-def3-11e6-bf01-fe55135034f3", "version": "01.02.010", "uri": "../lciamethods/b5c614d2-def3-11e6-bf01-fe55135034f3.xml"}, "meanAmount": 0.0, "other": {"anies": [{"value": "0.0138", "module": "A1", "scenario": "Standard Scenarios"}, {"value": "0.001471844", "module": "A2", "scenario": "Standard Scenarios"}, {"value": "0.00102021629593", "module": "A3", "scenario": "Standard Scenarios"}, {"value": "0.01629206029593", "module": "A1-A3", "scenario": "Standard Scenarios"}, {"value": "0.0", "module": "C1", "scenario": "Standard Scenarios"}, {"value": "9.123E-6", "module": "C2", "scenario": "Standard Scenarios"}, {"value": "0.0", "module": "C3", "scenario": "Standard Scenarios"}, {"value": "1.8197729863E-4", "module": "C4", "scenario": "Standard Scenarios"}, {"value": "-4.7586248217E-4", "module": "D", "scenario": "Standard Scenarios"}, {"name": "referenceToUnitGroupDataSet", "value": {"shortDescription": [{"value": "mol N-eq.", "lang": "en"}], "type": "unit group data set", "refObjectId": "71b4d617-0ec9-4d3f-b65e-e438940c2401", "version": "00.00.003", "uri": "../unitgroups/71b4d617-0ec9-4d3f-b65e-e438940c2401.xml"}}]}}, {"referenceToLCIAMethodDataSet": {"shortDescription": [{"value": "Potential Comparative Toxic Unit for ecosystems (ETP-fw)", "lang": "en"}, {"value": "Potenzielle Toxizitätsvergleichseinheit für Ökosysteme (ETP-fw)", "lang": "de"}], "type": "LCIA method data set", "refObjectId": "ee1082d1-b0f7-43ca-a1f0-21e2a4a74511", "version": "01.00.003", "uri": "../lciamethods/ee1082d1-b0f7-43ca-a1f0-21e2a4a74511.xml"}, "meanAmount": 0.0, "other": {"anies": [{"value": "0.0", "module": "A1", "scenario": "Standard Scenarios"}, {"value": "0.87845274", "module": "A2", "scenario": "Standard Scenarios"}, {"value": "0.78455220598436", "module": "A3", "scenario": "Standard Scenarios"}, {"value": "1.66300494598436", "module": "A1-A3", "scenario": "Standard Scenarios"}, {"value": "0.0", "module": "C1", "scenario": "Standard Scenarios"}, {"value": "0.005444955", "module": "C2", "scenario": "Standard Scenarios"}, {"value": "0.0", "module": "C3", "scenario": "Standard Scenarios"}, {"value": "0.09167936883103", "module": "C4", "scenario": "Standard Scenarios"}, {"value": "-1.9099127928472", "module": "D", "scenario": "Standard Scenarios"}, {"name": "referenceToUnitGroupDataSet", "value": {"shortDescription": [{"value": "CTUe", "lang": "en"}], "type": "unit group data set", "refObjectId": "aa959ded-f1eb-4efb-9c5c-2d60be36b3e6", "version": "00.00.003", "uri": "../unitgroups/aa959ded-f1eb-4efb-9c5c-2d60be36b3e6.xml"}}]}}, {"referenceToLCIAMethodDataSet": {"shortDescription": [{"value": "Global Warming Potential - biogenic (GWP-biogenic)", "lang": "en"}, {"value": "Globales Erwärmungspotenzial - biogen (GWP-biogenic)", "lang": "de"}], "type": "LCIA method data set", "refObjectId": "2356e1ab-0185-4db5-86e5-16de51c7485c", "version": "01.00.006", "uri": "../lciamethods/2356e1ab-0185-4db5-86e5-16de51c7485c.xml"}, "meanAmount": 0.0, "other": {"anies": [{"value": "0.00412", "module": "A1", "scenario": "Standard Scenarios"}, {"value": "2.63296E-5", "module": "A2", "scenario": "Standard Scenarios"}, {"value": "-5.2695937043E-4", "module": "A3", "scenario": "Standard Scenarios"}, {"value": "0.00361937022957", "module": "A1-A3", "scenario": "Standard Scenarios"}, {"value": "0.0", "module": "C1", "scenario": "Standard Scenarios"}, {"value": "1.632E-7", "module": "C2", "scenario": "Standard Scenarios"}, {"value": "0.0", "module": "C3", "scenario": "Standard Scenarios"}, {"value": "3.1945816E-6", "module": "C4", "scenario": "Standard Scenarios"}, {"value": "8.498115261E-5", "module": "D", "scenario": "Standard Scenarios"}, {"name": "referenceToUnitGroupDataSet", "value": {"shortDescription": [{"value": "kg CO2-eq.", "lang": "en"}], "type": "unit group data set", "refObjectId": "1ebf3012-d0db-4de2-aefd-ef30cedb0be1", "version": "30.00.000", "uri": "../unitgroups/1ebf3012-d0db-4de2-aefd-ef30cedb0be1.xml"}}]}}, {"referenceToLCIAMethodDataSet": {"shortDescription": [{"value": "Global Warming Potential - fossil fuels (GWP-fossil)", "lang": "en"}, {"value": "Globales Erwärmungspotenzial - fossil (GWP-fossil)", "lang": "de"}], "type": "LCIA method data set", "refObjectId": "5f635281-343e-44fb-83df-1971b155e6b6", "version": "01.00.009", "uri": "../lciamethods/5f635281-343e-44fb-83df-1971b155e6b6.xml"}, "meanAmount": 0.0, "other": {"anies": [{"value": "1.58", "module": "A1", "scenario": "Standard Scenarios"}, {"value": "0.065317736", "module": "A2", "scenario": "Standard Scenarios"}, {"value": "0.16472439780683", "module": "A3", "scenario": "Standard Scenarios"}, {"value": "1.81004213380683", "module": "A1-A3", "scenario": "Standard Scenarios"}, {"value": "0.0", "module": "C1", "scenario": "Standard Scenarios"}, {"value": "4.04862E-4", "module": "C2", "scenario": "Standard Scenarios"}, {"value": "0.0", "module": "C3", "scenario": "Standard Scenarios"}, {"value": "0.0050548975346", "module": "C4", "scenario": "Standard Scenarios"}, {"value": "-0.05698674288579", "module": "D", "scenario": "Standard Scenarios"}, {"name": "referenceToUnitGroupDataSet", "value": {"shortDescription": [{"value": "kg CO2-eq.", "lang": "en"}], "type": "unit group data set", "refObjectId": "1ebf3012-d0db-4de2-aefd-ef30cedb0be1", "version": "30.00.000", "uri": "../unitgroups/1ebf3012-d0db-4de2-aefd-ef30cedb0be1.xml"}}]}}, {"referenceToLCIAMethodDataSet": {"shortDescription": [{"value": "Global Warming Potential - land use and land use change (GWP-luluc)", "lang": "en"}, {"value": "Globales Erwärmungspotenzial - luluc (GWP-luluc)", "lang": "de"}], "type": "LCIA method data set", "refObjectId": "4331bbdb-978a-490d-8707-eeb047f01a55", "version": "01.00.006", "uri": "../lciamethods/4331bbdb-978a-490d-8707-eeb047f01a55.xml"}, "meanAmount": 0.0, "other": {"anies": [{"value": "2.92E-4", "module": "A1", "scenario": "Standard Scenarios"}, {"value": "2.3958E-5", "module": "A2", "scenario": "Standard Scenarios"}, {"value": "6.537956974E-5", "module": "A3", "scenario": "Standard Scenarios"}, {"value": "3.8133756973999995E-4", "module": "A1-A3", "scenario": "Standard Scenarios"}, {"value": "0.0", "module": "C1", "scenario": "Standard Scenarios"}, {"value": "1.485E-7", "module": "C2", "scenario": "Standard Scenarios"}, {"value": "0.0", "module": "C3", "scenario": "Standard Scenarios"}, {"value": "1.40917918E-6", "module": "C4", "scenario": "Standard Scenarios"}, {"value": "4.20763065E-5", "module": "D", "scenario": "Standard Scenarios"}, {"name": "referenceToUnitGroupDataSet", "value": {"shortDescription": [{"value": "kg CO2-eq.", "lang": "en"}], "type": "unit group data set", "refObjectId": "1ebf3012-d0db-4de2-aefd-ef30cedb0be1", "version": "30.00.000", "uri": "../unitgroups/1ebf3012-d0db-4de2-aefd-ef30cedb0be1.xml"}}]}}, {"referenceToLCIAMethodDataSet": {"shortDescription": [{"value": "Global Warming Potential - total (GWP-total)", "lang": "en"}, {"value": "Globales Erwärmungspotenzial - total (GWP-total)", "lang": "de"}], "type": "LCIA method data set", "refObjectId": "6a37f984-a4b3-458a-a20a-64418c145fa2", "version": "04.00.017", "uri": "../lciamethods/6a37f984-a4b3-458a-a20a-64418c145fa2.xml"}, "meanAmount": 0.0, "other": {"anies": [{"value": "1.93", "module": "A1", "scenario": "Standard Scenarios"}, {"value": "0.065368072", "module": "A2", "scenario": "Standard Scenarios"}, {"value": "0.1739392615271", "module": "A3", "scenario": "Standard Scenarios"}, {"value": "2.1693073335271", "module": "A1-A3", "scenario": "Standard Scenarios"}, {"value": "0.0", "module": "C1", "scenario": "Standard Scenarios"}, {"value": "4.05174E-4", "module": "C2", "scenario": "Standard Scenarios"}, {"value": "0.0", "module": "C3", "scenario": "Standard Scenarios"}, {"value": "0.00505950129538", "module": "C4", "scenario": "Standard Scenarios"}, {"value": "-0.05685968542669", "module": "D", "scenario": "Standard Scenarios"}, {"name": "referenceToUnitGroupDataSet", "value": {"shortDescription": [{"value": "kg CO2-eq.", "lang": "en"}], "type": "unit group data set", "refObjectId": "1ebf3012-d0db-4de2-aefd-ef30cedb0be1", "version": "30.00.000", "uri": "../unitgroups/1ebf3012-d0db-4de2-aefd-ef30cedb0be1.xml"}}]}}, {"referenceToLCIAMethodDataSet": {"shortDescription": [{"value": "Potential Comparative Toxic Unit for humans - cancer effects (HTP-c)", "lang": "en"}, {"value": "Potenzielle Toxizitätsvergleichseinheit für den Menschen - kanzerogene Wirkung (HTP-c)", "lang": "de"}], "type": "LCIA method data set", "refObjectId": "2299222a-bbd8-474f-9d4f-4dd1f18aea7c", "version": "01.00.004", "uri": "../lciamethods/2299222a-bbd8-474f-9d4f-4dd1f18aea7c.xml"}, "meanAmount": 0.0, "other": {"anies": [{"value": "0.0", "module": "A1", "scenario": "Standard Scenarios"}, {"value": "2.851E-11", "module": "A2", "scenario": "Standard Scenarios"}, {"value": "7.075E-11", "module": "A3", "scenario": "Standard Scenarios"}, {"value": "9.926E-11", "module": "A1-A3", "scenario": "Standard Scenarios"}, {"value": "0.0", "module": "C1", "scenario": "Standard Scenarios"}, {"value": "1.8E-13", "module": "C2", "scenario": "Standard Scenarios"}, {"value": "0.0", "module": "C3", "scenario": "Standard Scenarios"}, {"value": "2.12E-12", "module": "C4", "scenario": "Standard Scenarios"}, {"value": "-7.37E-12", "module": "D", "scenario": "Standard Scenarios"}, {"name": "referenceToUnitGroupDataSet", "value": {"shortDescription": [{"value": "CTUh", "lang": "en"}], "type": "unit group data set", "refObjectId": "d4c9523e-2d7e-49fd-8469-998f547d3a70", "version": "00.00.003", "uri": "../unitgroups/d4c9523e-2d7e-49fd-8469-998f547d3a70.xml"}}]}}, {"referenceToLCIAMethodDataSet": {"shortDescription": [{"value": "Potential Comparative Toxic Unit for humans - non-cancer effects (HTP-nc)", "lang": "en"}, {"value": "Potenzielle Toxizitätsvergleichseinheit für den Menschen - nicht kanzerogene Wirkung (HTP-nc)", "lang": "de"}], "type": "LCIA method data set", "refObjectId": "3af763a5-b7a1-48c9-9cee-1f223481fcef", "version": "01.00.003", "uri": "../lciamethods/3af763a5-b7a1-48c9-9cee-1f223481fcef.xml"}, "meanAmount": 0.0, "other": {"anies": [{"value": "0.0", "module": "A1", "scenario": "Standard Scenarios"}, {"value": "9.6316E-10", "module": "A2", "scenario": "Standard Scenarios"}, {"value": "2.50783E-9", "module": "A3", "scenario": "Standard Scenarios"}, {"value": "3.4709900000000002E-9", "module": "A1-A3", "scenario": "Standard Scenarios"}, {"value": "0.0", "module": "C1", "scenario": "Standard Scenarios"}, {"value": "5.97E-12", "module": "C2", "scenario": "Standard Scenarios"}, {"value": "0.0", "module": "C3", "scenario": "Standard Scenarios"}, {"value": "6.515E-11", "module": "C4", "scenario": "Standard Scenarios"}, {"value": "1.103884E-8", "module": "D", "scenario": "Standard Scenarios"}, {"name": "referenceToUnitGroupDataSet", "value": {"shortDescription": [{"value": "CTUh", "lang": "en"}], "type": "unit group data set", "refObjectId": "d4c9523e-2d7e-49fd-8469-998f547d3a70", "version": "00.00.003", "uri": "../unitgroups/d4c9523e-2d7e-49fd-8469-998f547d3a70.xml"}}]}}, {"referenceToLCIAMethodDataSet": {"shortDescription": [{"value": "Potential Human exposure efficiency relative to U235 (IRP)", "lang": "en"}, {"value": "Potenzielle Wirkung durch Exposition des Menschen mit U235 (IRP)", "lang": "de"}], "type": "LCIA method data set", "refObjectId": "b5c632be-def3-11e6-bf01-fe55135034f3", "version": "01.00.012", "uri": "../lciamethods/b5c632be-def3-11e6-bf01-fe55135034f3.xml"}, "meanAmount": 0.0, "other": {"anies": [{"value": "0.0", "module": "A1", "scenario": "Standard Scenarios"}, {"value": "0.004127552", "module": "A2", "scenario": "Standard Scenarios"}, {"value": "0.00598567833305", "module": "A3", "scenario": "Standard Scenarios"}, {"value": "0.01011323033305", "module": "A1-A3", "scenario": "Standard Scenarios"}, {"value": "0.0", "module": "C1", "scenario": "Standard Scenarios"}, {"value": "2.5584E-5", "module": "C2", "scenario": "Standard Scenarios"}, {"value": "0.0", "module": "C3", "scenario": "Standard Scenarios"}, {"value": "5.797627826E-4", "module": "C4", "scenario": "Standard Scenarios"}, {"value": "9.7381904193E-4", "module": "D", "scenario": "Standard Scenarios"}, {"name": "referenceToUnitGroupDataSet", "value": {"shortDescription": [{"value": "kgBq U235-eq.", "lang": "en"}], "type": "unit group data set", "refObjectId": "456b05bf-1415-44a9-9993-02452f554c09", "version": "00.00.003", "uri": "../unitgroups/456b05bf-1415-44a9-9993-02452f554c09.xml"}}]}}, {"referenceToLCIAMethodDataSet": {"shortDescription": [{"value": "Depletion potential of the stratospheric ozone layer (ODP)", "lang": "en"}, {"value": "Abbaupotenzial der stratosphärischen Ozonschicht (ODP)", "lang": "de"}], "type": "LCIA method data set", "refObjectId": "b5c629d6-def3-11e6-bf01-fe55135034f3", "version": "02.00.013", "uri": "../lciamethods/b5c629d6-def3-11e6-bf01-fe55135034f3.xml"}, "meanAmount": 0.0, "other": {"anies": [{"value": "2.16E-7", "module": "A1", "scenario": "Standard Scenarios"}, {"value": "1.44232E-8", "module": "A2", "scenario": "Standard Scenarios"}, {"value": "2.048116E-8", "module": "A3", "scenario": "Standard Scenarios"}, {"value": "2.5090436E-7", "module": "A1-A3", "scenario": "Standard Scenarios"}, {"value": "0.0", "module": "C1", "scenario": "Standard Scenarios"}, {"value": "8.94E-11", "module": "C2", "scenario": "Standard Scenarios"}, {"value": "0.0", "module": "C3", "scenario": "Standard Scenarios"}, {"value": "2.08175E-9", "module": "C4", "scenario": "Standard Scenarios"}, {"value": "-1.39084E-9", "module": "D", "scenario": "Standard Scenarios"}, {"name": "referenceToUnitGroupDataSet", "value": {"shortDescription": [{"value": "kg CFC-11-eq.", "lang": "en"}], "type": "unit group data set", "refObjectId": "d9e957c9-7309-4474-bf3a-7777df6c4e5b", "version": "25.00.000", "uri": "../unitgroups/d9e957c9-7309-4474-bf3a-7777df6c4e5b.xml"}}]}}, {"referenceToLCIAMethodDataSet": {"shortDescription": [{"value": "Potential incidence of disease due to PM emissions (PM)", "lang": "en"}, {"value": "Potenzielles Auftreten von Krankheiten aufgrund von Feinstaubemissionen (PM)", "lang": "de"}], "type": "LCIA method data set", "refObjectId": "b5c602c6-def3-11e6-bf01-fe55135034f3", "version": "02.00.012", "uri": "../lciamethods/b5c602c6-def3-11e6-bf01-fe55135034f3.xml"}, "meanAmount": 0.0, "other": {"anies": [{"value": "0.0", "module": "A1", "scenario": "Standard Scenarios"}, {"value": "5.8564E-9", "module": "A2", "scenario": "Standard Scenarios"}, {"value": "2.01609E-9", "module": "A3", "scenario": "Standard Scenarios"}, {"value": "7.87249E-9", "module": "A1-A3", "scenario": "Standard Scenarios"}, {"value": "0.0", "module": "C1", "scenario": "Standard Scenarios"}, {"value": "3.63E-11", "module": "C2", "scenario": "Standard Scenarios"}, {"value": "0.0", "module": "C3", "scenario": "Standard Scenarios"}, {"value": "9.3279E-10", "module": "C4", "scenario": "Standard Scenarios"}, {"value": "-3.29893E-9", "module": "D", "scenario": "Standard Scenarios"}, {"name": "referenceToUnitGroupDataSet", "value": {"shortDescription": [{"value": "Disease incidence", "lang": "en"}], "type": "unit group data set", "refObjectId": "3883559b-648f-4afc-8ba2-0bd24f3affa3", "version": "00.00.003", "uri": "../unitgroups/3883559b-648f-4afc-8ba2-0bd24f3affa3.xml"}}]}}, {"referenceToLCIAMethodDataSet": {"shortDescription": [{"value": "Photochemical Ozone Creation Potential (POCP)", "lang": "en"}, {"value": "Bildungspotenzial für troposphärisches Ozon (POCP)", "lang": "de"}], "type": "LCIA method data set", "refObjectId": "b5c610fe-def3-11e6-bf01-fe55135034f3", "version": "02.00.015", "uri": "../lciamethods/b5c610fe-def3-11e6-bf01-fe55135034f3.xml"}, "meanAmount": 0.0, "other": {"anies": [{"value": "0.00456", "module": "A1", "scenario": "Standard Scenarios"}, {"value": "4.20112E-4", "module": "A2", "scenario": "Standard Scenarios"}, {"value": "6.2968254995E-4", "module": "A3", "scenario": "Standard Scenarios"}, {"value": "0.00560979454995", "module": "A1-A3", "scenario": "Standard Scenarios"}, {"value": "0.0", "module": "C1", "scenario": "Standard Scenarios"}, {"value": "2.604E-6", "module": "C2", "scenario": "Standard Scenarios"}, {"value": "0.0", "module": "C3", "scenario": "Standard Scenarios"}, {"value": "5.285888443E-5", "module": "C4", "scenario": "Standard Scenarios"}, {"value": "-3.2381768691E-4", "module": "D", "scenario": "Standard Scenarios"}, {"name": "referenceToUnitGroupDataSet", "value": {"shortDescription": [{"value": "kg NMVOC-eq.", "lang": "en"}], "type": "unit group data set", "refObjectId": "d27c25f8-fbc1-44c6-b47b-4adbae4199c6", "version": "00.00.003", "uri": "../unitgroups/d27c25f8-fbc1-44c6-b47b-4adbae4199c6.xml"}}]}}, {"referenceToLCIAMethodDataSet": {"shortDescription": [{"value": "Potential Soil quality index (SQP)", "lang": "en"}, {"value": "Potenzieller Bodenqualitätsindex (SQP)", "lang": "de"}], "type": "LCIA method data set", "refObjectId": "b2ad6890-c78d-11e6-9d9d-cec0c932ce01", "version": "01.00.011", "uri": "../lciamethods/b2ad6890-c78d-11e6-9d9d-cec0c932ce01.xml"}, "meanAmount": 0.0, "other": {"anies": [{"value": "0.0", "module": "A1", "scenario": "Standard Scenarios"}, {"value": "0.854338408", "module": "A2", "scenario": "Standard Scenarios"}, {"value": "0.38880195491686", "module": "A3", "scenario": "Standard Scenarios"}, {"value": "1.24314036291686", "module": "A1-A3", "scenario": "Standard Scenarios"}, {"value": "0.0", "module": "C1", "scenario": "Standard Scenarios"}, {"value": "0.005295486", "module": "C2", "scenario": "Standard Scenarios"}, {"value": "0.0", "module": "C3", "scenario": "Standard Scenarios"}, {"value": "0.29639400065804", "module": "C4", "scenario": "Standard Scenarios"}, {"value": "-0.08796020035192", "module": "D", "scenario": "Standard Scenarios"}, {"name": "referenceToUnitGroupDataSet", "value": {"shortDescription": [{"value": "dimensionless", "lang": "en"}], "type": "unit group data set", "refObjectId": "f130951c-e67f-4f7f-8dd4-665de3974e18", "version": "00.00.004", "uri": "../unitgroups/f130951c-e67f-4f7f-8dd4-665de3974e18.xml"}}]}}, {"referenceToLCIAMethodDataSet": {"shortDescription": [{"value": "Water (user) deprivation potential (WDP)", "lang": "en"}, {"value": "Wasser-Entzugspotenzial (Benutzer) (WDP)", "lang": "de"}], "type": "LCIA method data set", "refObjectId": "b2ad66ce-c78d-11e6-9d9d-cec0c932ce01", "version": "03.00.015", "uri": "../lciamethods/b2ad66ce-c78d-11e6-9d9d-cec0c932ce01.xml"}, "meanAmount": 0.0, "other": {"anies": [{"value": "74.8", "module": "A1", "scenario": "Standard Scenarios"}, {"value": "0.003524488", "module": "A2", "scenario": "Standard Scenarios"}, {"value": "2.10464209709601", "module": "A3", "scenario": "Standard Scenarios"}, {"value": "76.908166585096", "module": "A1-A3", "scenario": "Standard Scenarios"}, {"value": "0.0", "module": "C1", "scenario": "Standard Scenarios"}, {"value": "2.1846E-5", "module": "C2", "scenario": "Standard Scenarios"}, {"value": "0.0", "module": "C3", "scenario": "Standard Scenarios"}, {"value": "0.00633521828871", "module": "C4", "scenario": "Standard Scenarios"}, {"value": "-0.01086431535472", "module": "D", "scenario": "Standard Scenarios"}, {"name": "referenceToUnitGroupDataSet", "value": {"shortDescription": [{"value": "m3 world eq. deprived", "lang": "en"}], "type": "unit group data set", "refObjectId": "6ae2df01-888e-46c8-b17d-49fa3869b476", "version": "00.00.003", "uri": "../unitgroups/6ae2df01-888e-46c8-b17d-49fa3869b476.xml"}}]}}]}, "otherAttributes": {"{http://www.indata.network/EPD/2019}epd-version": "1.2"}, "version": "1.1"}