{"processInformation": {"dataSetInformation": {"UUID": "60b31769-fae7-4d5d-ae00-ad5a6a39468a", "name": {"baseName": [{"value": "Promatect-MST®, Promatect-MT®, Promarine 450T®, Promarine 640T®, Supalux M1®, Vermiculux T®, Promatect-MLT®, Promasil® 1100 Super and Promasil® 1000L", "lang": "en"}, {"value": "Promatect-MST®, Promatect-MT®, Promarine 450T®, Promarine 640T®, Supalux M1®, Vermiculux T®, Promatect-MLT®, Promasil 1100 super und Promasil 1000L", "lang": "de"}], "functionalUnitFlowProperties": [{"lang": "en"}]}, "classificationInformation": {"classification": [{"class": [{"value": "Dämmstoffe", "level": 0, "classId": "2"}, {"value": "Calciumsilikat / Calcium-Silikathydrat", "level": 1, "classId": "2.20"}, {"value": "Calciumsilikat", "level": 2, "classId": "2.20.02"}], "name": "OEKOBAU.DAT"}, {"class": [{"value": "02 Building products", "level": 0}, {"value": "Thermal insulation products", "level": 1}, {"value": "Calcium silicate insulating materials", "level": 2}], "name": "IBUCategories"}]}, "generalComment": [{"value": "Promatect-MST®, Promarine 450T®, Promarine 640T®, Supalux M1®, Promatect-MT®, Vermiculux T®, Promatect-MLT®, Promasil® 1100 Super and Promasil® 1000L.\nThis EPD describes the life cycle analysis of different Promat products for fire protection. The product ranges under consideration are the cement-bounded medium-density calcium silicate fire protective boards. In detail, the investigated products are 9 for this range, including Promatect MT®, Promatect MST®, Promatect MLT®, Promarine 450T®, Promarine 640T®, Supalux M1®, Vermiculux T®, Promasil® 1100 Super and Promasil® 1000L. \nThe boards are self-supporting, non-combustible, asbestos-free and moisture-resistant calcium silicate fire protection boards for a variety of applications. The products differentiate by individual densities and the ratios of included raw materials to meet the technical requirements of individual applications. \nThe function of these fire protective boards is generally equal being the provision of structural fire protection. This can be by covering walls, floorings, and ceilings in buildings, by covering structural steelwork or by constructing fire-resistant ducts and same applications apply to Promarine boards within the Marine sector.", "lang": "en"}, {"value": "Promatect-MST®, Promarine 450T®, Promarine 640T®, Supalux M1®, Promatect-MT®, Vermiculux T®, Promatect-MLT®, Promasil 1100super und Promasil 1000L Diese EPD beschreibt die Lebenszyklusanalyse von verschiedenen Promat-Produkten für den Brandschutz. Bei den betrachteten Produktreihen handelt es sich um zementgebundene Calciumsilikat-Brandschutzplatten mittlerer Dichte. Im Einzelnen handelt es sich bei den untersuchten Produkten um 9 für diese Produktreihe, darunter Promatect MT, Promatect MST, Promatect MLT, Promarine 450T, Promarine 640T, Supalux M1, Vermiculux T, Promasil 1100super und Promasil 1000L. \nDie Platten sind selbsttragende, nicht kombinierbare, asbestfreie und feuchtigkeitsbeständige Kalziumsilikat-Brandschutzplatten für eine Vielzahl von Anwendungen. Die Produkte unterscheiden sich durch individuelle Dichten und das Verhältnis der enthaltenen Rohstoffe, um den technischen Anforderungen der einzelnen Anwendungen gerecht zu werden. \nDie Funktion dieser Brandschutzplatten ist im Allgemeinen die Bereitstellung eines baulichen Brandschutzes. Dies kann durch die Verkleidung von Wänden, Böden und Decken in Gebäuden, durch die Verkleidung von Stahlkonstruktionen oder durch den Bau von feuerfesten Kanälen geschehen. Die gleichen Anwendungen gelten für Promarine-Platten im Bereich der Schifffahrt.", "lang": "de"}], "other": {"anies": [{"scenario": [{"description": [{"value": "100% recycling", "lang": "en"}, {"value": "100% Recycling", "lang": "de"}], "name": "S1"}, {"description": [{"value": "100% landfill", "lang": "en"}, {"value": "100% Deponierung", "lang": "de"}], "name": "S2", "default": true}]}]}}, "quantitativeReference": {"referenceToReferenceFlow": [0]}, "time": {"referenceYear": 2024, "dataSetValidUntil": 2028, "other": {"anies": [{"name": "publicationDateOfEPD", "value": 1712534400000}]}}, "geography": {"locationOfOperationSupplyOrProduction": {"location": "RER"}}, "technology": {"technologyDescriptionAndIncludedProcesses": [{"value": "There is only one manufacturing plant of the declared products being the manufacturing plant in Tisselt (Belgium). The products are all produced on the same type of production line. All raw materials, including previously made xonotlite slurries, together with a balanced amount of water are mixed to form a slurry, and shaped by a filter press to produce a wet board. It is steam cured in an autoclave to form required calcium silicate minerals suitable for the end application. Final steps are the drying, cutting and sanding/finishing. During the cutting and finishing, scrap is produced which is partly recycled, both internally and externally, and partly landfilled. \nDeclared unit: \n1 m2 of Promatect-MST® with a thickness of 40 mm.", "lang": "en"}, {"value": "Es gibt nur eine einzige Produktionsstätte für die angegebenen Produkte, nämlich die Produktionsstätte in Tisselt (Belgien). Die Produkte werden alle auf der gleichen Art von Produktionslinie hergestellt. Alle Rohstoffe, einschließlich der zuvor hergestellten Xonotlit-Schlämme, werden zusammen mit einer ausgewogenen Menge Wasser zu einem Schlamm gemischt und durch eine Filterpresse zu einer Nassplatte geformt. Diese wird in einem Autoklaven dampfgehärtet, um die für die Endanwendung geeigneten Kalziumsilikatmineralien zu bilden. \nTechnische Daten: \n sehen die pdf technischendaten tabelle \nDeklarierte Einheit: \n1 m2 Promatect-MST® mit einer Dicke von 40 mm.", "lang": "de"}], "technologicalApplicability": [{"value": "Promatect-MST®, Supalux M1®, Promatect-MT®, Vermiculux T®, Promatect-MLT® boards are versatile multi-purpose fire protection boards, for multiple applications:\nFIRE-RATED ASSEMBLIES: Building and industrial construction, among other things for fire dampers and smoke extraction dampers, fire doors and metal profile insulator\nPromarine 450T®, Promarine 640T®\n\nA, B & C Class divisions\nCompartmentations\nLinings\nNon-combustible furniture\n\nPromasil® 1100 Super and Promasil® 1000L\nAluminium industry: anode baking furnace and electrolysis cells\nSteel industry: smelting and heat treatment furnaces\nGlass industry: melting furnaces, heat treatment and foming furnaces\nCeramics industry: bogie hearth furnaces, kiln cars\nCement industry: heat exchangers and cyclone separators\n\nOil and gas industry: fired heaters pipe supports", "lang": "en"}, {"value": "Promatect-MST®, Supalux M1®, Promatect-MT®, Vermiculux T®, Promatect-MLT® sind vielseitige Mehrzweck-Brandschutzplatten, für zahlreiche Anwendungen BRANDSCHUTZMONTAGE: Hoch- und Industriebau, u.a. für Brandschutz- und Entrauchungsklappen, Brandschutztüren und Metallprofilisolatoren Promarine 450T®, Promarine 640T®, A, B & C Klasse Trennwände Auskleidungen Nicht brennbare Möbel Promasil 1100 super und Promasil 1000L Aluminiumindustrie: Anodenbrennöfen und Elektrolysezellen Stahlindustrie: Schmelz- und Wärmebehandlungsöfen Glasindustrie: Schmelzöfen, Wärmebehandlungs- und Brennöfen Keramikindustrie: Herdwagenöfen, Ofenwagen Zementindustrie: Wärmetauscher und Zyklonabscheider Öl- und Gasindustrie: befeuerte Heizungen Rohrhalterungen", "lang": "de"}]}}, "modellingAndValidation": {"LCIMethodAndAllocation": {"typeOfDataSet": "EPD", "referenceToLCAMethodDetails": [{"shortDescription": [{"value": "Calcium silicate insulating materials.pdf", "lang": "en"}], "type": "source data set", "refObjectId": "27209ed5-4408-4290-a2b6-5daf221f7f38"}], "other": {"anies": [{"name": "subType", "value": "representative dataset"}]}}, "dataSourcesTreatmentAndRepresentativeness": {"referenceToDataSource": [{"shortDescription": [{"value": "ecoinvent database (all versions)", "lang": "en"}], "type": "source data set", "refObjectId": "b497a91f-e14b-4b69-8f28-f50eb1576766"}, {"shortDescription": [{"value": "ecoinvent 3.8 database", "lang": "en"}], "type": "source data set", "refObjectId": "0f4c65c0-6210-450f-b886-82bf8dd5ace9"}], "useAdviceForDataSet": [{"value": "Scope: \nThis EPD is representative and relevant for Promatect-MST®, Promarine 450T®, Promarine 640T®, Supalux M1®, Promatect-MT®, Vermiculux T®, Promatect-MLT®, Promasil® 1100 Super and Promasil® 1000L boards produced by ETEX in Tisselt (Belgium) and installed in Europe. The data describing the direct inputs and outputs of the foreground processes are representative for ETEX production in Tisselt, Belgium, and taken from the period of one year between October 2020 and September 2021.\n\nThe results in this EPD are based on Promatect-MST®. In the LCA background report the representativeness of Promatect-MST® has been checked by comparing the LCA results of Promatect-MST® with the LCA results of the other products included in the scope of the EPD. \nSystem boundary: \nCradle-to-gate with options, including modules C2-C4 and D", "lang": "en"}, {"value": "Gültigkeitsbereich: \nDiese EPD ist repräsentativ und relevant für Promatect-MST®, Promarine 450T®, Promarine 640T®, Supalux M1®, Promatect-MT®, Vermiculux T®, Promatect-MLT®, Promasil 1100 super und Promasil 1000L Platten, die von ETEX in Tisselt (Belgien) hergestellt und in Europa installiert werden. Die Daten, die die direkten Inputs und Outputs der Vordergrundprozesse beschreiben, sind repräsentativ für die ETEX-Produktion in Tisselt, Belgien, und stammen aus dem Zeitraum eines Jahres zwischen Oktober 2020 und September 2021. Die Ergebnisse in dieser EPD basieren auf Promatect-MST®. Im LCA-Hintergrundbericht wurde die Repräsentativität von Promatect-MST® überprüft, indem die LCA-Ergebnisse von Promatect-MST® mit den LCA-Ergebnissen der anderen Produkte im Rahmen der EPD verglichen wurden. \nSystemgrenze: \nCradle-to-Gate mit Optionen, einschließlich Modul C2-C4 und D", "lang": "de"}], "other": {"anies": [{"name": "referenceToOriginalEPD", "value": {"shortDescription": {"value": "Promatect-MST®, Promatect-MT®, Promarine 450T®, Promarine 640T®, Supalux M1®, Vermiculux T®, Promatect-MLT®, Promasil® 1100 Super and Promasil® 1000L.pdf", "defaultValue": "Promatect-MST®, Promatect-MT®, Promarine 450T®, Promarine 640T®, Supalux M1®, Vermiculux T®, Promatect-MLT®, Promasil® 1100 Super and Promasil® 1000L.pdf", "lstrings": [{"lang": "en", "value": "Promatect-MST®, Promatect-MT®, Promarine 450T®, Promarine 640T®, Supalux M1®, Vermiculux T®, Promatect-MLT®, Promasil® 1100 Super and Promasil® 1000L.pdf"}]}, "type": "source data set", "uuid": {"uuid": "650bc291-3dc8-414a-957b-38fe096d7e80"}, "refObjectId": "650bc291-3dc8-414a-957b-38fe096d7e80", "resourceURLs": ["https://oekobaudat.de/OEKOBAU.DAT/resource/sources/650bc291-3dc8-414a-957b-38fe096d7e80/Promatect-MST_Promatect-MT_Promarine_450T_Promarine_640T_Supalux_M1_Vermiculux_T_Promatect-MLT_Promasil_1100_Super_and_Promasil_1000L_20068.pdf?version=00.02.000"]}}]}}, "validation": {"review": [{"referenceToNameOfReviewerAndInstitution": [{"shortDescription": [{"value": "Institut Bauen und Umwelt e. V.", "lang": "en"}], "type": "contact data set", "refObjectId": "d111dbec-b024-4be5-86c5-752d6eb2cf95", "uri": "../contacts/d111dbec-b024-4be5-86c5-752d6eb2cf95.xml"}], "type": "Accredited third party review"}]}, "complianceDeclarations": {"compliance": [{"referenceToComplianceSystem": {"shortDescription": [{"value": "DIN EN 15804+A2", "lang": "en"}], "type": "source data set", "refObjectId": "c0016b33-8cf7-415c-ac6e-deba0d21440d", "uri": "../sources/c0016b33-8cf7-415c-ac6e-deba0d21440d.xml"}}, {"referenceToComplianceSystem": {"shortDescription": [{"value": "ISO 14025", "lang": "en"}], "type": "source data set", "refObjectId": "4f2eb655-6e44-4874-a95a-e28f5442cd4d", "uri": "../sources/4f2eb655-6e44-4874-a95a-e28f5442cd4d.xml"}}]}}, "administrativeInformation": {"commissionerAndGoal": {"referenceToCommissioner": [{"shortDescription": [{"value": "Etex Building Performance International", "lang": "en"}], "type": "contact data set", "refObjectId": "9f15c029-1fb0-467d-8dd1-92b013e91ca8", "uri": "../contacts/9f15c029-1fb0-467d-8dd1-92b013e91ca8.xml"}]}, "dataGenerator": {"referenceToPersonOrEntityGeneratingTheDataSet": [{"shortDescription": [{"value": "Enperas", "lang": "en"}], "type": "contact data set", "refObjectId": "71c3ddb3-f20b-4161-af33-52bc33b3106d", "uri": "../contacts/71c3ddb3-f20b-4161-af33-52bc33b3106d.xml"}]}, "dataEntryBy": {"timeStamp": 1712534400000, "referenceToDataSetFormat": [{"shortDescription": [{"value": "ILCD Format", "lang": "en"}], "type": "source data set", "refObjectId": "a97a0155-0234-4b87-b4ce-a45da52f2a40", "uri": "../sources/a97a0155-0234-4b87-b4ce-a45da52f2a40.xml"}, {"shortDescription": [{"value": "EPD-Datenformaterweiterungen v1.2", "lang": "de"}, {"value": "EPD Data Format Extensions v1.2", "lang": "en"}], "type": "source data set", "refObjectId": "a29449fd-aa2f-4de8-b5d7-4b06b43c6fde", "uri": "../sources/a29449fd-aa2f-4de8-b5d7-4b06b43c6fde.xml"}]}, "publicationAndOwnership": {"dataSetVersion": "00.04.000", "referenceToRegistrationAuthority": {"shortDescription": [{"value": "Institut Bauen und Umwelt e. V.", "lang": "en"}], "type": "contact data set", "refObjectId": "d111dbec-b024-4be5-86c5-752d6eb2cf95", "uri": "../contacts/d111dbec-b024-4be5-86c5-752d6eb2cf95.xml"}, "registrationNumber": "EPD-ETE-20230253-IBA2-EN", "referenceToOwnershipOfDataSet": {"shortDescription": [{"value": "Etex Building Performance International", "lang": "en"}], "type": "contact data set", "refObjectId": "9f15c029-1fb0-467d-8dd1-92b013e91ca8", "uri": "../contacts/9f15c029-1fb0-467d-8dd1-92b013e91ca8.xml"}, "copyright": true, "licenseType": "Free of charge for all users and uses", "accessRestrictions": [{"value": "None", "lang": "en"}], "other": {"anies": [{"name": "referenceToPublisher", "value": {"shortDescription": [{"value": "Institut Bauen und Umwelt e. V.", "lang": "en"}], "type": "contact data set", "refObjectId": "d111dbec-b024-4be5-86c5-752d6eb2cf95", "uri": "../contacts/d111dbec-b024-4be5-86c5-752d6eb2cf95.xml"}}]}}}, "exchanges": {"exchange": [{"dataSetInternalID": 0, "referenceToFlowDataSet": {"shortDescription": [{"value": "Promatect-MST®, Promarine 450T®, Promarine 640T®, Supalux M1®, Promatect-MT®, Vermiculux T®, Promatect-MLT® (1 m2 Promatect-MST® mit einer Dicke von 40 mm.)", "lang": "en"}], "type": "flow data set", "refObjectId": "63f7ff2d-a7f3-c272-b39a-dd468b11984e", "uri": "../flows/63f7ff2d-a7f3-c272-b39a-dd468b11984e.xml"}, "meanAmount": 1.0, "referencesToDataSource": {}, "referenceFlow": true, "resolvedFlowVersion": "00.04.000", "resultingflowAmount": 1.0, "flowProperties": [{"name": [{"lang": "de", "value": "Fläche"}, {"lang": "en", "value": "Area"}], "uuid": "93a60a56-a3c8-19da-a746-0800200c9a66", "referenceFlowProperty": true, "meanValue": 1.0, "referenceUnit": "qm", "unitGroupUUID": "c20a03d7-bd90-4569-bc94-66cfd364dfc8"}], "materialProperties": [{"name": "grammage", "value": "36.58", "unit": "kg/m^2", "unitDescription": "kilograms per square meter"}, {"name": "gross density", "value": "750.0", "unit": "kg/m^3", "unitDescription": "kilograms per cubic metre"}, {"name": "layer thickness", "value": "0.04", "unit": "m", "unitDescription": "meters"}], "typeOfFlow": "Product flow", "classification": {"classHierarchy": "Dämmstoffe / Calciumsilikat / Calcium-Silikathydrat / Calciumsilikat", "name": "OEKOBAU.DAT"}}, {"dataSetInternalID": 1, "referenceToFlowDataSet": {"shortDescription": [{"value": "Renewable primary energy as energy carrier (PERE)", "lang": "en"}, {"value": "Erneuerbare Primärenergie als Energieträger (PERE)", "lang": "de"}], "type": "flow data set", "refObjectId": "20f32be5-0398-4288-9b6d-accddd195317", "uri": "../flows/20f32be5-0398-4288-9b6d-accddd195317.xml"}, "exchange direction": "INPUT", "other": {"anies": [{"name": "referenceToUnitGroupDataSet", "value": {"shortDescription": [{"value": "MJ", "lang": "en"}], "type": "unit group data set", "refObjectId": "93a60a57-a3c8-11da-a746-0800200c9a66", "uri": "../unitgroups/93a60a57-a3c8-11da-a746-0800200c9a66.xml"}}, {"value": "61.9389", "module": "A1-A3"}, {"value": "4.466", "module": "A5"}, {"value": "0.06078", "module": "C2", "scenario": "S1"}, {"value": "0.05352", "module": "C2", "scenario": "S2"}, {"value": "1.082", "module": "C3", "scenario": "S1"}, {"value": "0", "module": "C3", "scenario": "S2"}, {"value": "0", "module": "C4", "scenario": "S1"}, {"value": "0.2683", "module": "C4", "scenario": "S2"}, {"value": "0", "module": "D", "scenario": "S1"}, {"value": "0", "module": "D", "scenario": "S2"}]}, "resolvedFlowVersion": "38.00.000", "flowProperties": [], "typeOfFlow": "Other flow", "classification": {"classHierarchy": "Quantities", "name": "GaBiCategories"}}, {"dataSetInternalID": 2, "referenceToFlowDataSet": {"shortDescription": [{"value": "Renewable primary energy resources as material utilization (PERM)", "lang": "en"}, {"value": "Erneuerbare Primärenergie zur stofflichen Nutzung (PERM)", "lang": "de"}], "type": "flow data set", "refObjectId": "fb3ec0de-548d-4508-aea5-00b73bf6f702", "uri": "../flows/fb3ec0de-548d-4508-aea5-00b73bf6f702.xml"}, "exchange direction": "INPUT", "other": {"anies": [{"name": "referenceToUnitGroupDataSet", "value": {"shortDescription": [{"value": "MJ", "lang": "en"}], "type": "unit group data set", "refObjectId": "93a60a57-a3c8-11da-a746-0800200c9a66", "uri": "../unitgroups/93a60a57-a3c8-11da-a746-0800200c9a66.xml"}}, {"value": "41.08", "module": "A1-A3"}, {"value": "-9.263", "module": "A5"}, {"value": "0", "module": "C2", "scenario": "S1"}, {"value": "0", "module": "C2", "scenario": "S2"}, {"value": "-19.67", "module": "C3", "scenario": "S1"}, {"value": "0", "module": "C3", "scenario": "S2"}, {"value": "0", "module": "C4", "scenario": "S1"}, {"value": "0", "module": "C4", "scenario": "S2"}, {"value": "24.48", "module": "D", "scenario": "S1"}, {"value": "4.814", "module": "D", "scenario": "S2"}]}, "resolvedFlowVersion": "38.00.000", "flowProperties": [], "typeOfFlow": "Other flow", "classification": {"classHierarchy": "Quantities", "name": "GaBiCategories"}}, {"dataSetInternalID": 3, "referenceToFlowDataSet": {"shortDescription": [{"value": "Total use of renewable primary energy resources (PERT)", "lang": "en"}, {"value": "Total erneuerbare Primärenergie (PERT)", "lang": "de"}], "type": "flow data set", "refObjectId": "53f97275-fa8a-4cdd-9024-65936002acd0", "uri": "../flows/53f97275-fa8a-4cdd-9024-65936002acd0.xml"}, "exchange direction": "INPUT", "other": {"anies": [{"name": "referenceToUnitGroupDataSet", "value": {"shortDescription": [{"value": "MJ", "lang": "en"}], "type": "unit group data set", "refObjectId": "93a60a57-a3c8-11da-a746-0800200c9a66", "uri": "../unitgroups/93a60a57-a3c8-11da-a746-0800200c9a66.xml"}}, {"value": "103.0289", "module": "A1-A3"}, {"value": "-4.799", "module": "A5"}, {"value": "0.06078", "module": "C2", "scenario": "S1"}, {"value": "0.05352", "module": "C2", "scenario": "S2"}, {"value": "-18.4", "module": "C3", "scenario": "S1"}, {"value": "0", "module": "C3", "scenario": "S2"}, {"value": "0", "module": "C4", "scenario": "S1"}, {"value": "0.2683", "module": "C4", "scenario": "S2"}, {"value": "24.48", "module": "D", "scenario": "S1"}, {"value": "4.814", "module": "D", "scenario": "S2"}]}, "resolvedFlowVersion": "38.00.000", "flowProperties": [], "typeOfFlow": "Other flow", "classification": {"classHierarchy": "Quantities / Environmental quantities / EPD EN 15804 / LCI indicators", "name": "GaBiCategories"}}, {"dataSetInternalID": 4, "referenceToFlowDataSet": {"shortDescription": [{"value": "Non renewable primary energy as energy carrier (PENRE)", "lang": "en"}, {"value": "Nicht-erneuerbare Primärenergie als Energieträger (PENRE)", "lang": "de"}], "type": "flow data set", "refObjectId": "ac857178-2b45-46ec-892a-a9a4332f0372", "uri": "../flows/ac857178-2b45-46ec-892a-a9a4332f0372.xml"}, "exchange direction": "INPUT", "other": {"anies": [{"name": "referenceToUnitGroupDataSet", "value": {"shortDescription": [{"value": "MJ", "lang": "en"}], "type": "unit group data set", "refObjectId": "93a60a57-a3c8-11da-a746-0800200c9a66", "uri": "../unitgroups/93a60a57-a3c8-11da-a746-0800200c9a66.xml"}}, {"value": "401.9", "module": "A1-A3"}, {"value": "0.57", "module": "A5"}, {"value": "4.347", "module": "C2", "scenario": "S1"}, {"value": "3.828", "module": "C2", "scenario": "S2"}, {"value": "7.512", "module": "C3", "scenario": "S1"}, {"value": "0", "module": "C3", "scenario": "S2"}, {"value": "0", "module": "C4", "scenario": "S1"}, {"value": "5.334", "module": "C4", "scenario": "S2"}, {"value": "0", "module": "D", "scenario": "S1"}, {"value": "0", "module": "D", "scenario": "S2"}]}, "resolvedFlowVersion": "38.00.000", "flowProperties": [], "typeOfFlow": "Other flow", "classification": {"classHierarchy": "Quantities", "name": "GaBiCategories"}}, {"dataSetInternalID": 5, "referenceToFlowDataSet": {"shortDescription": [{"value": "Non renewable primary energy as material utilization (PENRM)", "lang": "en"}, {"value": "Nicht-erneuerbare Primärenergie zur stofflichen Nutzung (PENRM)", "lang": "de"}], "type": "flow data set", "refObjectId": "1421caa0-679d-4bf4-b282-0eb850ccae27", "uri": "../flows/1421caa0-679d-4bf4-b282-0eb850ccae27.xml"}, "exchange direction": "INPUT", "other": {"anies": [{"name": "referenceToUnitGroupDataSet", "value": {"shortDescription": [{"value": "MJ", "lang": "en"}], "type": "unit group data set", "refObjectId": "93a60a57-a3c8-11da-a746-0800200c9a66", "uri": "../unitgroups/93a60a57-a3c8-11da-a746-0800200c9a66.xml"}}, {"value": "0.1184", "module": "A1-A3"}, {"value": "-0.07228", "module": "A5"}, {"value": "0", "module": "C2", "scenario": "S1"}, {"value": "0", "module": "C2", "scenario": "S2"}, {"value": "0", "module": "C3", "scenario": "S1"}, {"value": "0", "module": "C3", "scenario": "S2"}, {"value": "0", "module": "C4", "scenario": "S1"}, {"value": "0", "module": "C4", "scenario": "S2"}, {"value": "0.03415", "module": "D", "scenario": "S1"}, {"value": "0.03415", "module": "D", "scenario": "S2"}]}, "resolvedFlowVersion": "38.00.000", "flowProperties": [], "typeOfFlow": "Other flow", "classification": {"classHierarchy": "Quantities", "name": "GaBiCategories"}}, {"dataSetInternalID": 6, "referenceToFlowDataSet": {"shortDescription": [{"value": "Total use of non renewable primary energy resources (PENRT)", "lang": "en"}, {"value": "Total nicht erneuerbare Primärenergie (PENRT)", "lang": "de"}], "type": "flow data set", "refObjectId": "06159210-646b-4c8d-8583-da9b3b95a6c1", "uri": "../flows/06159210-646b-4c8d-8583-da9b3b95a6c1.xml"}, "exchange direction": "INPUT", "other": {"anies": [{"name": "referenceToUnitGroupDataSet", "value": {"shortDescription": [{"value": "MJ", "lang": "en"}], "type": "unit group data set", "refObjectId": "93a60a57-a3c8-11da-a746-0800200c9a66", "uri": "../unitgroups/93a60a57-a3c8-11da-a746-0800200c9a66.xml"}}, {"value": "402", "module": "A1-A3"}, {"value": "0.4761", "module": "A5"}, {"value": "4.347", "module": "C2", "scenario": "S1"}, {"value": "3.828", "module": "C2", "scenario": "S2"}, {"value": "8.764", "module": "C3", "scenario": "S1"}, {"value": "0", "module": "C3", "scenario": "S2"}, {"value": "0", "module": "C4", "scenario": "S1"}, {"value": "5.334", "module": "C4", "scenario": "S2"}, {"value": "0.03415", "module": "D", "scenario": "S1"}, {"value": "0.03415", "module": "D", "scenario": "S2"}]}, "resolvedFlowVersion": "38.00.000", "flowProperties": [], "typeOfFlow": "Other flow", "classification": {"classHierarchy": "Quantities / Environmental quantities / EPD EN 15804 / LCI indicators", "name": "GaBiCategories"}}, {"dataSetInternalID": 7, "referenceToFlowDataSet": {"shortDescription": [{"value": "Use of secondary material (SM)", "lang": "en"}, {"value": "Einsatz von Sekundärstoffen (SM)", "lang": "de"}], "type": "flow data set", "refObjectId": "c6a1f35f-2d09-4f54-8dfb-97e502e1ce92", "uri": "../flows/c6a1f35f-2d09-4f54-8dfb-97e502e1ce92.xml"}, "exchange direction": "INPUT", "other": {"anies": [{"name": "referenceToUnitGroupDataSet", "value": {"shortDescription": [{"value": "kg", "lang": "en"}], "type": "unit group data set", "refObjectId": "ad38d542-3fe9-439d-9b95-2f5f7752acaf", "uri": "../unitgroups/ad38d542-3fe9-439d-9b95-2f5f7752acaf.xml"}}, {"value": "0.058", "module": "A1-A3"}, {"value": "0", "module": "A5"}, {"value": "0", "module": "C2", "scenario": "S1"}, {"value": "0", "module": "C2", "scenario": "S2"}, {"value": "0", "module": "C3", "scenario": "S1"}, {"value": "0", "module": "C3", "scenario": "S2"}, {"value": "0", "module": "C4", "scenario": "S1"}, {"value": "0", "module": "C4", "scenario": "S2"}, {"value": "0", "module": "D", "scenario": "S1"}, {"value": "0", "module": "D", "scenario": "S2"}]}, "resolvedFlowVersion": "38.00.000", "flowProperties": [], "typeOfFlow": "Other flow", "classification": {"classHierarchy": "Quantities / Environmental quantities / EPD EN 15804 / LCI indicators", "name": "GaBiCategories"}}, {"dataSetInternalID": 8, "referenceToFlowDataSet": {"shortDescription": [{"value": "Use of renewable secondary fuels (RSF)", "lang": "en"}, {"value": "Erneuerbare Sekundärbrennstoffe (RSF)", "lang": "de"}], "type": "flow data set", "refObjectId": "64333088-a55f-4aa2-9a31-c10b07816787", "uri": "../flows/64333088-a55f-4aa2-9a31-c10b07816787.xml"}, "exchange direction": "INPUT", "other": {"anies": [{"name": "referenceToUnitGroupDataSet", "value": {"shortDescription": [{"value": "MJ", "lang": "en"}], "type": "unit group data set", "refObjectId": "93a60a57-a3c8-11da-a746-0800200c9a66", "uri": "../unitgroups/93a60a57-a3c8-11da-a746-0800200c9a66.xml"}}, {"value": "0", "module": "A1-A3"}, {"value": "0", "module": "A5"}, {"value": "0", "module": "C2", "scenario": "S1"}, {"value": "0", "module": "C2", "scenario": "S2"}, {"value": "0", "module": "C3", "scenario": "S1"}, {"value": "0", "module": "C3", "scenario": "S2"}, {"value": "0", "module": "C4", "scenario": "S1"}, {"value": "0", "module": "C4", "scenario": "S2"}, {"value": "0", "module": "D", "scenario": "S1"}, {"value": "0", "module": "D", "scenario": "S2"}]}, "resolvedFlowVersion": "38.00.000", "flowProperties": [], "typeOfFlow": "Other flow", "classification": {"classHierarchy": "Quantities / Environmental quantities / EPD EN 15804 / LCI indicators", "name": "GaBiCategories"}}, {"dataSetInternalID": 9, "referenceToFlowDataSet": {"shortDescription": [{"value": "Use of non renewable secondary fuels (NRSF)", "lang": "en"}, {"value": "Nicht erneuerbare Sekundärbrennstoffe (NRSF)", "lang": "de"}], "type": "flow data set", "refObjectId": "89def144-d39a-4287-b86f-efde453ddcb2", "uri": "../flows/89def144-d39a-4287-b86f-efde453ddcb2.xml"}, "exchange direction": "INPUT", "other": {"anies": [{"name": "referenceToUnitGroupDataSet", "value": {"shortDescription": [{"value": "MJ", "lang": "en"}], "type": "unit group data set", "refObjectId": "93a60a57-a3c8-11da-a746-0800200c9a66", "uri": "../unitgroups/93a60a57-a3c8-11da-a746-0800200c9a66.xml"}}, {"value": "0", "module": "A1-A3"}, {"value": "0", "module": "A5"}, {"value": "0", "module": "C2", "scenario": "S1"}, {"value": "0", "module": "C2", "scenario": "S2"}, {"value": "0", "module": "C3", "scenario": "S1"}, {"value": "0", "module": "C3", "scenario": "S2"}, {"value": "0", "module": "C4", "scenario": "S1"}, {"value": "0", "module": "C4", "scenario": "S2"}, {"value": "0", "module": "D", "scenario": "S1"}, {"value": "0", "module": "D", "scenario": "S2"}]}, "resolvedFlowVersion": "38.00.000", "flowProperties": [], "typeOfFlow": "Other flow", "classification": {"classHierarchy": "Quantities / Environmental quantities / EPD EN 15804 / LCI indicators", "name": "GaBiCategories"}}, {"dataSetInternalID": 10, "referenceToFlowDataSet": {"shortDescription": [{"value": "Use of net fresh water (FW)", "lang": "en"}, {"value": "Einsatz von Süßwasserressourcen (FW)", "lang": "de"}], "type": "flow data set", "refObjectId": "3cf952c8-f3a4-461d-8c96-96456ca62246", "uri": "../flows/3cf952c8-f3a4-461d-8c96-96456ca62246.xml"}, "exchange direction": "INPUT", "other": {"anies": [{"name": "referenceToUnitGroupDataSet", "value": {"shortDescription": [{"value": "m^3", "lang": "en"}], "type": "unit group data set", "refObjectId": "cd950537-0a98-4044-9ba7-9f9a68d0a504", "uri": "../unitgroups/cd950537-0a98-4044-9ba7-9f9a68d0a504.xml"}}, {"value": "0.2780293", "module": "A1-A3"}, {"value": "0.0002991", "module": "A5"}, {"value": "0.0003179", "module": "C2", "scenario": "S1"}, {"value": "0.00028", "module": "C2", "scenario": "S2"}, {"value": "0.00621", "module": "C3", "scenario": "S1"}, {"value": "0", "module": "C3", "scenario": "S2"}, {"value": "0", "module": "C4", "scenario": "S1"}, {"value": "0.005588", "module": "C4", "scenario": "S2"}, {"value": "-0.006103", "module": "D", "scenario": "S1"}, {"value": "-0.001866", "module": "D", "scenario": "S2"}]}, "resolvedFlowVersion": "38.00.000", "flowProperties": [], "typeOfFlow": "Other flow", "classification": {"classHierarchy": "Quantities / Environmental quantities / EPD EN 15804 / LCI indicators", "name": "GaBiCategories"}}, {"dataSetInternalID": 11, "referenceToFlowDataSet": {"shortDescription": [{"value": "Hazardous waste disposed (HWD)", "lang": "en"}, {"value": "Gefährlicher Abfall zur Deponie (HWD)", "lang": "de"}], "type": "flow data set", "refObjectId": "430f9e0f-59b2-46a0-8e0d-55e0e84948fc", "uri": "../flows/430f9e0f-59b2-46a0-8e0d-55e0e84948fc.xml"}, "exchange direction": "OUTPUT", "other": {"anies": [{"name": "referenceToUnitGroupDataSet", "value": {"shortDescription": [{"value": "kg", "lang": "en"}], "type": "unit group data set", "refObjectId": "ad38d542-3fe9-439d-9b95-2f5f7752acaf", "uri": "../unitgroups/ad38d542-3fe9-439d-9b95-2f5f7752acaf.xml"}}, {"value": "0.00047692", "module": "A1-A3"}, {"value": "1.146E-06", "module": "A5"}, {"value": "1.128E-05", "module": "C2", "scenario": "S1"}, {"value": "9.937E-06", "module": "C2", "scenario": "S2"}, {"value": "4.029E-06", "module": "C3", "scenario": "S1"}, {"value": "0", "module": "C3", "scenario": "S2"}, {"value": "0", "module": "C4", "scenario": "S1"}, {"value": "5.695E-06", "module": "C4", "scenario": "S2"}, {"value": "-1.571E-05", "module": "D", "scenario": "S1"}, {"value": "-3.94E-06", "module": "D", "scenario": "S2"}]}, "resolvedFlowVersion": "38.00.000", "flowProperties": [], "typeOfFlow": "Other flow", "classification": {"classHierarchy": "Quantities / Environmental quantities / EPD EN 15804 / LCI indicators", "name": "GaBiCategories"}}, {"dataSetInternalID": 12, "referenceToFlowDataSet": {"shortDescription": [{"value": "Non hazardous waste disposed (NHWD)", "lang": "en"}, {"value": "Entsorgter nicht gefährlicher Abfall (NHWD)", "lang": "de"}], "type": "flow data set", "refObjectId": "b29ef66b-e286-4afa-949f-62f1a7b4d7fa", "uri": "../flows/b29ef66b-e286-4afa-949f-62f1a7b4d7fa.xml"}, "exchange direction": "OUTPUT", "other": {"anies": [{"name": "referenceToUnitGroupDataSet", "value": {"shortDescription": [{"value": "kg", "lang": "en"}], "type": "unit group data set", "refObjectId": "ad38d542-3fe9-439d-9b95-2f5f7752acaf", "uri": "../unitgroups/ad38d542-3fe9-439d-9b95-2f5f7752acaf.xml"}}, {"value": "5.2212", "module": "A1-A3"}, {"value": "0.4071", "module": "A5"}, {"value": "0.2264", "module": "C2", "scenario": "S1"}, {"value": "0.1994", "module": "C2", "scenario": "S2"}, {"value": "0.05045", "module": "C3", "scenario": "S1"}, {"value": "0", "module": "C3", "scenario": "S2"}, {"value": "0", "module": "C4", "scenario": "S1"}, {"value": "29.99", "module": "C4", "scenario": "S2"}, {"value": "-0.04055", "module": "D", "scenario": "S1"}, {"value": "-0.01935", "module": "D", "scenario": "S2"}]}, "resolvedFlowVersion": "38.00.000", "flowProperties": [], "typeOfFlow": "Other flow", "classification": {"classHierarchy": "Quantities / Environmental quantities / EPD EN 15804 / LCI indicators", "name": "GaBiCategories"}}, {"dataSetInternalID": 13, "referenceToFlowDataSet": {"shortDescription": [{"value": "Radioactive waste disposed (RWD)", "lang": "en"}, {"value": "Entsorgter radioaktiver Abfall (RWD)", "lang": "de"}], "type": "flow data set", "refObjectId": "3449546e-52ad-4b39-b809-9fb77cea8ff6", "uri": "../flows/3449546e-52ad-4b39-b809-9fb77cea8ff6.xml"}, "exchange direction": "OUTPUT", "other": {"anies": [{"name": "referenceToUnitGroupDataSet", "value": {"shortDescription": [{"value": "kg", "lang": "en"}], "type": "unit group data set", "refObjectId": "ad38d542-3fe9-439d-9b95-2f5f7752acaf", "uri": "../unitgroups/ad38d542-3fe9-439d-9b95-2f5f7752acaf.xml"}}, {"value": "0.0007319", "module": "A1-A3"}, {"value": "3.221E-06", "module": "A5"}, {"value": "2.921E-05", "module": "C2", "scenario": "S1"}, {"value": "2.572E-05", "module": "C2", "scenario": "S2"}, {"value": "5.3E-05", "module": "C3", "scenario": "S1"}, {"value": "0", "module": "C3", "scenario": "S2"}, {"value": "0", "module": "C4", "scenario": "S1"}, {"value": "3.551E-05", "module": "C4", "scenario": "S2"}, {"value": "-5.372E-05", "module": "D", "scenario": "S1"}, {"value": "-1.243E-05", "module": "D", "scenario": "S2"}]}, "resolvedFlowVersion": "38.00.000", "flowProperties": [], "typeOfFlow": "Other flow", "classification": {"classHierarchy": "Quantities / Environmental quantities / EPD EN 15804 / LCI indicators", "name": "GaBiCategories"}}, {"dataSetInternalID": 14, "referenceToFlowDataSet": {"shortDescription": [{"value": "Components for re-use (CRU)", "lang": "en"}, {"value": "Komponenten für die Wiederverwendung (CRU)", "lang": "de"}], "type": "flow data set", "refObjectId": "a2b32f97-3fc7-4af2-b209-525bc6426f33", "uri": "../flows/a2b32f97-3fc7-4af2-b209-525bc6426f33.xml"}, "exchange direction": "OUTPUT", "other": {"anies": [{"name": "referenceToUnitGroupDataSet", "value": {"shortDescription": [{"value": "kg", "lang": "en"}], "type": "unit group data set", "refObjectId": "ad38d542-3fe9-439d-9b95-2f5f7752acaf", "uri": "../unitgroups/ad38d542-3fe9-439d-9b95-2f5f7752acaf.xml"}}, {"value": "0", "module": "A1-A3"}, {"value": "0", "module": "A5"}, {"value": "0", "module": "C2", "scenario": "S1"}, {"value": "0", "module": "C2", "scenario": "S2"}, {"value": "0", "module": "C3", "scenario": "S1"}, {"value": "0", "module": "C3", "scenario": "S2"}, {"value": "0", "module": "C4", "scenario": "S1"}, {"value": "0", "module": "C4", "scenario": "S2"}, {"value": "0", "module": "D", "scenario": "S1"}, {"value": "0", "module": "D", "scenario": "S2"}]}, "resolvedFlowVersion": "38.00.000", "flowProperties": [], "typeOfFlow": "Other flow", "classification": {"classHierarchy": "Quantities / Environmental quantities / EPD EN 15804 / LCI indicators", "name": "GaBiCategories"}}, {"dataSetInternalID": 15, "referenceToFlowDataSet": {"shortDescription": [{"value": "Materials for recycling (MFR)", "lang": "en"}, {"value": "Stoffe zum Recycling (MFR)", "lang": "de"}], "type": "flow data set", "refObjectId": "d7fe48a5-4103-49c8-9aae-b0b5dfdbd6ae", "uri": "../flows/d7fe48a5-4103-49c8-9aae-b0b5dfdbd6ae.xml"}, "exchange direction": "OUTPUT", "other": {"anies": [{"name": "referenceToUnitGroupDataSet", "value": {"shortDescription": [{"value": "kg", "lang": "en"}], "type": "unit group data set", "refObjectId": "ad38d542-3fe9-439d-9b95-2f5f7752acaf", "uri": "../unitgroups/ad38d542-3fe9-439d-9b95-2f5f7752acaf.xml"}}, {"value": "0", "module": "A1-A3"}, {"value": "0.3395", "module": "A5"}, {"value": "0", "module": "C2", "scenario": "S1"}, {"value": "0", "module": "C2", "scenario": "S2"}, {"value": "30", "module": "C3", "scenario": "S1"}, {"value": "0", "module": "C3", "scenario": "S2"}, {"value": "0", "module": "C4", "scenario": "S1"}, {"value": "0", "module": "C4", "scenario": "S2"}, {"value": "0", "module": "D", "scenario": "S1"}, {"value": "0", "module": "D", "scenario": "S2"}]}, "resolvedFlowVersion": "38.00.000", "flowProperties": [], "typeOfFlow": "Other flow", "classification": {"classHierarchy": "Quantities / Environmental quantities / EPD EN 15804 / LCI indicators", "name": "GaBiCategories"}}, {"dataSetInternalID": 16, "referenceToFlowDataSet": {"shortDescription": [{"value": "Materials for energy recovery (MER)", "lang": "en"}, {"value": "Stoffe für die Energierückgewinnung (MER)", "lang": "de"}], "type": "flow data set", "refObjectId": "59a9181c-3aaf-46ee-8b13-2b3723b6e447", "uri": "../flows/59a9181c-3aaf-46ee-8b13-2b3723b6e447.xml"}, "exchange direction": "OUTPUT", "other": {"anies": [{"name": "referenceToUnitGroupDataSet", "value": {"shortDescription": [{"value": "kg", "lang": "en"}], "type": "unit group data set", "refObjectId": "ad38d542-3fe9-439d-9b95-2f5f7752acaf", "uri": "../unitgroups/ad38d542-3fe9-439d-9b95-2f5f7752acaf.xml"}}, {"value": "0", "module": "A1-A3"}, {"value": "0", "module": "A5"}, {"value": "0", "module": "C2", "scenario": "S1"}, {"value": "0", "module": "C2", "scenario": "S2"}, {"value": "0", "module": "C3", "scenario": "S1"}, {"value": "0", "module": "C3", "scenario": "S2"}, {"value": "0", "module": "C4", "scenario": "S1"}, {"value": "0", "module": "C4", "scenario": "S2"}, {"value": "0", "module": "D", "scenario": "S1"}, {"value": "0", "module": "D", "scenario": "S2"}]}, "resolvedFlowVersion": "38.00.000", "flowProperties": [], "typeOfFlow": "Other flow", "classification": {"classHierarchy": "Quantities / Environmental quantities / EPD EN 15804 / LCI indicators", "name": "GaBiCategories"}}, {"dataSetInternalID": 17, "referenceToFlowDataSet": {"shortDescription": [{"value": "Exported electrical energy (EEE)", "lang": "en"}, {"value": "Exportierte elektrische Energie (EEE)", "lang": "de"}], "type": "flow data set", "refObjectId": "4da0c987-2b76-40d6-9e9e-82a017aaaf29", "uri": "../flows/4da0c987-2b76-40d6-9e9e-82a017aaaf29.xml"}, "exchange direction": "OUTPUT", "other": {"anies": [{"name": "referenceToUnitGroupDataSet", "value": {"shortDescription": [{"value": "MJ", "lang": "en"}], "type": "unit group data set", "refObjectId": "93a60a57-a3c8-11da-a746-0800200c9a66", "uri": "../unitgroups/93a60a57-a3c8-11da-a746-0800200c9a66.xml"}}, {"value": "0", "module": "A1-A3"}, {"value": "0.4487", "module": "A5"}, {"value": "0", "module": "C2", "scenario": "S1"}, {"value": "0", "module": "C2", "scenario": "S2"}, {"value": "0", "module": "C3", "scenario": "S1"}, {"value": "0", "module": "C3", "scenario": "S2"}, {"value": "0", "module": "C4", "scenario": "S1"}, {"value": "0", "module": "C4", "scenario": "S2"}, {"value": "0", "module": "D", "scenario": "S1"}, {"value": "0", "module": "D", "scenario": "S2"}]}, "resolvedFlowVersion": "38.00.000", "flowProperties": [], "typeOfFlow": "Other flow", "classification": {"classHierarchy": "Quantities / Environmental quantities / EPD EN 15804 / LCI indicators", "name": "GaBiCategories"}}, {"dataSetInternalID": 18, "referenceToFlowDataSet": {"shortDescription": [{"value": "Exported thermal energy (EET)", "lang": "en"}, {"value": "Exportierte thermische Energie (EET)", "lang": "de"}], "type": "flow data set", "refObjectId": "98daf38a-7a79-46d3-9a37-2b7bd0955810", "uri": "../flows/98daf38a-7a79-46d3-9a37-2b7bd0955810.xml"}, "exchange direction": "OUTPUT", "other": {"anies": [{"name": "referenceToUnitGroupDataSet", "value": {"shortDescription": [{"value": "MJ", "lang": "en"}], "type": "unit group data set", "refObjectId": "93a60a57-a3c8-11da-a746-0800200c9a66", "uri": "../unitgroups/93a60a57-a3c8-11da-a746-0800200c9a66.xml"}}, {"value": "0", "module": "A1-A3"}, {"value": "0.8974", "module": "A5"}, {"value": "0", "module": "C2", "scenario": "S1"}, {"value": "0", "module": "C2", "scenario": "S2"}, {"value": "0", "module": "C3", "scenario": "S1"}, {"value": "0", "module": "C3", "scenario": "S2"}, {"value": "0", "module": "C4", "scenario": "S1"}, {"value": "0", "module": "C4", "scenario": "S2"}, {"value": "0", "module": "D", "scenario": "S1"}, {"value": "0", "module": "D", "scenario": "S2"}]}, "resolvedFlowVersion": "38.00.000", "flowProperties": [], "typeOfFlow": "Other flow", "classification": {"classHierarchy": "Quantities / Environmental quantities / EPD EN 15804 / LCI indicators", "name": "GaBiCategories"}}]}, "LCIAResults": {"LCIAResult": [{"referenceToLCIAMethodDataSet": {"shortDescription": [{"value": "Global Warming Potential total (GWP-total)", "lang": "en"}, {"value": "Globales Erwärmungspotenzial total (GWP-total)", "lang": "de"}], "type": "LCIA method data set", "refObjectId": "6a37f984-a4b3-458a-a20a-64418c145fa2", "uri": "../lciamethods/6a37f984-a4b3-458a-a20a-64418c145fa2.xml"}, "other": {"anies": [{"name": "referenceToUnitGroupDataSet", "value": {"shortDescription": [{"value": "kg CO_(2) eq", "lang": "en"}], "type": "unit group data set", "refObjectId": "1ebf3012-d0db-4de2-aefd-ef30cedb0be1", "uri": "../unitgroups/1ebf3012-d0db-4de2-aefd-ef30cedb0be1.xml"}}, {"value": "28.065", "module": "A1-A3"}, {"value": "1.637", "module": "A5"}, {"value": "0.2854", "module": "C2", "scenario": "S1"}, {"value": "0.2513", "module": "C2", "scenario": "S2"}, {"value": "2.625", "module": "C3", "scenario": "S1"}, {"value": "0", "module": "C3", "scenario": "S2"}, {"value": "0", "module": "C4", "scenario": "S1"}, {"value": "2.437", "module": "C4", "scenario": "S2"}, {"value": "-1.228", "module": "D", "scenario": "S1"}, {"value": "-0.6699", "module": "D", "scenario": "S2"}]}}, {"referenceToLCIAMethodDataSet": {"shortDescription": [{"value": "Global Warming Potential fossil fuels (GWP-fossil)", "lang": "en"}, {"value": "Globales Erwärmungspotenzial fossil (GWP-fossil)", "lang": "de"}], "type": "LCIA method data set", "refObjectId": "5f635281-343e-44fb-83df-1971b155e6b6", "uri": "../lciamethods/5f635281-343e-44fb-83df-1971b155e6b6.xml"}, "other": {"anies": [{"name": "referenceToUnitGroupDataSet", "value": {"shortDescription": [{"value": "kg CO_(2) eq", "lang": "en"}], "type": "unit group data set", "refObjectId": "1ebf3012-d0db-4de2-aefd-ef30cedb0be1", "uri": "../unitgroups/1ebf3012-d0db-4de2-aefd-ef30cedb0be1.xml"}}, {"value": "32.633", "module": "A1-A3"}, {"value": "0.0362", "module": "A5"}, {"value": "0.2851", "module": "C2", "scenario": "S1"}, {"value": "0.2511", "module": "C2", "scenario": "S2"}, {"value": "0.3671", "module": "C3", "scenario": "S1"}, {"value": "0", "module": "C3", "scenario": "S2"}, {"value": "0", "module": "C4", "scenario": "S1"}, {"value": "0.1819", "module": "C4", "scenario": "S2"}, {"value": "-0.7134", "module": "D", "scenario": "S1"}, {"value": "-0.1574", "module": "D", "scenario": "S2"}]}}, {"referenceToLCIAMethodDataSet": {"shortDescription": [{"value": "Global Warming Potential biogenic (GWP-biogenic)", "lang": "en"}, {"value": "Globales Erwärmungspotenzial biogen (GWP-biogenic)", "lang": "de"}], "type": "LCIA method data set", "refObjectId": "2356e1ab-0185-4db5-86e5-16de51c7485c", "uri": "../lciamethods/2356e1ab-0185-4db5-86e5-16de51c7485c.xml"}, "other": {"anies": [{"name": "referenceToUnitGroupDataSet", "value": {"shortDescription": [{"value": "kg CO_(2) eq", "lang": "en"}], "type": "unit group data set", "refObjectId": "1ebf3012-d0db-4de2-aefd-ef30cedb0be1", "uri": "../unitgroups/1ebf3012-d0db-4de2-aefd-ef30cedb0be1.xml"}}, {"value": "-4.5785564", "module": "A1-A3"}, {"value": "1.598", "module": "A5"}, {"value": "0.000102", "module": "C2", "scenario": "S1"}, {"value": "8.982E-05", "module": "C2", "scenario": "S2"}, {"value": "2.256", "module": "C3", "scenario": "S1"}, {"value": "0", "module": "C3", "scenario": "S2"}, {"value": "0", "module": "C4", "scenario": "S1"}, {"value": "2.254", "module": "C4", "scenario": "S2"}, {"value": "-0.5128", "module": "D", "scenario": "S1"}, {"value": "-0.5115", "module": "D", "scenario": "S2"}]}}, {"referenceToLCIAMethodDataSet": {"shortDescription": [{"value": "Global Warming Potential luluc (GWP-luluc)", "lang": "en"}, {"value": "Globales Erwärmungspotenzial luluc (GWP-luluc)", "lang": "de"}], "type": "LCIA method data set", "refObjectId": "4331bbdb-978a-490d-8707-eeb047f01a55", "uri": "../lciamethods/4331bbdb-978a-490d-8707-eeb047f01a55.xml"}, "other": {"anies": [{"name": "referenceToUnitGroupDataSet", "value": {"shortDescription": [{"value": "kg CO_(2) eq", "lang": "en"}], "type": "unit group data set", "refObjectId": "1ebf3012-d0db-4de2-aefd-ef30cedb0be1", "uri": "../unitgroups/1ebf3012-d0db-4de2-aefd-ef30cedb0be1.xml"}}, {"value": "0.007862", "module": "A1-A3"}, {"value": "1.382E-05", "module": "A5"}, {"value": "0.000114", "module": "C2", "scenario": "S1"}, {"value": "0.0001004", "module": "C2", "scenario": "S2"}, {"value": "0.0007948", "module": "C3", "scenario": "S1"}, {"value": "0", "module": "C3", "scenario": "S2"}, {"value": "0", "module": "C4", "scenario": "S1"}, {"value": "0.0001341", "module": "C4", "scenario": "S2"}, {"value": "-0.001245", "module": "D", "scenario": "S1"}, {"value": "-0.0007033", "module": "D", "scenario": "S2"}]}}, {"referenceToLCIAMethodDataSet": {"shortDescription": [{"value": "Depletion potential of the stratospheric ozone layer (ODP)", "lang": "en"}, {"value": "Abbau Potential der stratosphärischen Ozonschicht (ODP)", "lang": "de"}], "type": "LCIA method data set", "refObjectId": "b5c629d6-def3-11e6-bf01-fe55135034f3", "uri": "../lciamethods/b5c629d6-def3-11e6-bf01-fe55135034f3.xml"}, "other": {"anies": [{"name": "referenceToUnitGroupDataSet", "value": {"shortDescription": [{"value": "kg CFC11 eq", "lang": "en"}], "type": "unit group data set", "refObjectId": "d9e957c9-7309-4474-bf3a-7777df6c4e5b", "uri": "../unitgroups/d9e957c9-7309-4474-bf3a-7777df6c4e5b.xml"}}, {"value": "3.5875E-06", "module": "A1-A3"}, {"value": "7.067E-09", "module": "A5"}, {"value": "6.607E-08", "module": "C2", "scenario": "S1"}, {"value": "5.818E-08", "module": "C2", "scenario": "S2"}, {"value": "2.797E-08", "module": "C3", "scenario": "S1"}, {"value": "0", "module": "C3", "scenario": "S2"}, {"value": "0", "module": "C4", "scenario": "S1"}, {"value": "6.736E-08", "module": "C4", "scenario": "S2"}, {"value": "-8.215E-08", "module": "D", "scenario": "S1"}, {"value": "-1.845E-08", "module": "D", "scenario": "S2"}]}}, {"referenceToLCIAMethodDataSet": {"shortDescription": [{"value": "Acidification potential of land and water (AP)", "lang": "en"}, {"value": "Versauerungspotenzial von Boden und Wasser (AP)", "lang": "de"}], "type": "LCIA method data set", "refObjectId": "b5c611c6-def3-11e6-bf01-fe55135034f3", "uri": "../lciamethods/b5c611c6-def3-11e6-bf01-fe55135034f3.xml"}, "other": {"anies": [{"name": "referenceToUnitGroupDataSet", "value": {"shortDescription": [{"value": "mol H^(+) eq", "lang": "en"}], "type": "unit group data set", "refObjectId": "42e089ac-92bf-4bf2-8ca1-5fc40d18f2ed", "uri": "../unitgroups/42e089ac-92bf-4bf2-8ca1-5fc40d18f2ed.xml"}}, {"value": "0.08829", "module": "A1-A3"}, {"value": "0.0002134", "module": "A5"}, {"value": "0.0008097", "module": "C2", "scenario": "S1"}, {"value": "0.000713", "module": "C2", "scenario": "S2"}, {"value": "0.00245", "module": "C3", "scenario": "S1"}, {"value": "0", "module": "C3", "scenario": "S2"}, {"value": "0", "module": "C4", "scenario": "S1"}, {"value": "0.001605", "module": "C4", "scenario": "S2"}, {"value": "-0.003623", "module": "D", "scenario": "S1"}, {"value": "-0.0006598", "module": "D", "scenario": "S2"}]}}, {"referenceToLCIAMethodDataSet": {"shortDescription": [{"value": "Eutrophication potential aquatic freshwater (EP-freshwater)", "lang": "en"}, {"value": "Eutrophierungspotenzial Süßwasser (EP-freshwater)", "lang": "de"}], "type": "LCIA method data set", "refObjectId": "b53ec18f-7377-4ad3-86eb-cc3f4f276b2b", "uri": "../lciamethods/b53ec18f-7377-4ad3-86eb-cc3f4f276b2b.xml"}, "other": {"anies": [{"name": "referenceToUnitGroupDataSet", "value": {"shortDescription": [{"value": "kg P eq", "lang": "en"}], "type": "unit group data set", "refObjectId": "0429039d-a61d-4590-ba67-aa4a20a810a1", "uri": "../unitgroups/0429039d-a61d-4590-ba67-aa4a20a810a1.xml"}}, {"value": "0.000242782", "module": "A1-A3"}, {"value": "3.895E-07", "module": "A5"}, {"value": "2.033E-06", "module": "C2", "scenario": "S1"}, {"value": "1.79E-06", "module": "C2", "scenario": "S2"}, {"value": "3.569E-05", "module": "C3", "scenario": "S1"}, {"value": "0", "module": "C3", "scenario": "S2"}, {"value": "0", "module": "C4", "scenario": "S1"}, {"value": "5.581E-06", "module": "C4", "scenario": "S2"}, {"value": "-3.486E-05", "module": "D", "scenario": "S1"}, {"value": "-1.091E-05", "module": "D", "scenario": "S2"}]}}, {"referenceToLCIAMethodDataSet": {"shortDescription": [{"value": "Eutrophication potential aquatic marine (EP-marine)", "lang": "en"}, {"value": "Eutrophierungspotenzial Salzwasser (EP-marine)", "lang": "de"}], "type": "LCIA method data set", "refObjectId": "b5c619fa-def3-11e6-bf01-fe55135034f3", "uri": "../lciamethods/b5c619fa-def3-11e6-bf01-fe55135034f3.xml"}, "other": {"anies": [{"name": "referenceToUnitGroupDataSet", "value": {"shortDescription": [{"value": "kg N eq", "lang": "en"}], "type": "unit group data set", "refObjectId": "d05bb823-ecdf-4686-8c40-bf1d9257859f", "uri": "../unitgroups/d05bb823-ecdf-4686-8c40-bf1d9257859f.xml"}}, {"value": "0.024415", "module": "A1-A3"}, {"value": "8.844E-05", "module": "A5"}, {"value": "0.0001609", "module": "C2", "scenario": "S1"}, {"value": "0.0001417", "module": "C2", "scenario": "S2"}, {"value": "0.0005278", "module": "C3", "scenario": "S1"}, {"value": "0", "module": "C3", "scenario": "S2"}, {"value": "0", "module": "C4", "scenario": "S1"}, {"value": "0.0005481", "module": "C4", "scenario": "S2"}, {"value": "-0.0009067", "module": "D", "scenario": "S1"}, {"value": "-0.0001595", "module": "D", "scenario": "S2"}]}}, {"referenceToLCIAMethodDataSet": {"shortDescription": [{"value": "Eutrophication potential terrestrial (EP-terrestrial)", "lang": "en"}, {"value": "Eutrophierungspotenzial Land (EP-terrestrial)", "lang": "de"}], "type": "LCIA method data set", "refObjectId": "b5c614d2-def3-11e6-bf01-fe55135034f3", "uri": "../lciamethods/b5c614d2-def3-11e6-bf01-fe55135034f3.xml"}, "other": {"anies": [{"name": "referenceToUnitGroupDataSet", "value": {"shortDescription": [{"value": "mol N eq", "lang": "en"}], "type": "unit group data set", "refObjectId": "71b4d617-0ec9-4d3f-b65e-e438940c2401", "uri": "../unitgroups/71b4d617-0ec9-4d3f-b65e-e438940c2401.xml"}}, {"value": "0.25952", "module": "A1-A3"}, {"value": "0.000877", "module": "A5"}, {"value": "0.001794", "module": "C2", "scenario": "S1"}, {"value": "0.001579", "module": "C2", "scenario": "S2"}, {"value": "0.005963", "module": "C3", "scenario": "S1"}, {"value": "0", "module": "C3", "scenario": "S2"}, {"value": "0", "module": "C4", "scenario": "S1"}, {"value": "0.006048", "module": "C4", "scenario": "S2"}, {"value": "-0.01172", "module": "D", "scenario": "S1"}, {"value": "-0.001759", "module": "D", "scenario": "S2"}]}}, {"referenceToLCIAMethodDataSet": {"shortDescription": [{"value": "Formation potential of tropospheric ozone photochemical oxidants (POCP)", "lang": "en"}, {"value": "Bildungspotential für troposphärisches Ozon (POCP)", "lang": "de"}], "type": "LCIA method data set", "refObjectId": "b5c610fe-def3-11e6-bf01-fe55135034f3", "uri": "../lciamethods/b5c610fe-def3-11e6-bf01-fe55135034f3.xml"}, "other": {"anies": [{"name": "referenceToUnitGroupDataSet", "value": {"shortDescription": [{"value": "kg NMVOC eq", "lang": "en"}], "type": "unit group data set", "refObjectId": "d27c25f8-fbc1-44c6-b47b-4adbae4199c6", "uri": "../unitgroups/d27c25f8-fbc1-44c6-b47b-4adbae4199c6.xml"}}, {"value": "0.07486", "module": "A1-A3"}, {"value": "0.0002592", "module": "A5"}, {"value": "0.0006894", "module": "C2", "scenario": "S1"}, {"value": "0.000607", "module": "C2", "scenario": "S2"}, {"value": "0.001588", "module": "C3", "scenario": "S1"}, {"value": "0", "module": "C3", "scenario": "S2"}, {"value": "0", "module": "C4", "scenario": "S1"}, {"value": "0.001722", "module": "C4", "scenario": "S2"}, {"value": "-0.002921", "module": "D", "scenario": "S1"}, {"value": "-0.0006132", "module": "D", "scenario": "S2"}]}}, {"referenceToLCIAMethodDataSet": {"shortDescription": [{"value": "Abiotic depletion potential for non fossil resources (ADPE)", "lang": "en"}, {"value": "Potenzial für den abiotischen Abbau nicht fossiler Ressourcen (ADPE)", "lang": "de"}], "type": "LCIA method data set", "refObjectId": "b2ad6494-c78d-11e6-9d9d-cec0c932ce01", "uri": "../lciamethods/b2ad6494-c78d-11e6-9d9d-cec0c932ce01.xml"}, "other": {"anies": [{"name": "referenceToUnitGroupDataSet", "value": {"shortDescription": [{"value": "kg Sb eq", "lang": "en"}], "type": "unit group data set", "refObjectId": "54ccd2d9-a32a-4fc2-923d-f2c8c93e89d4", "uri": "../unitgroups/54ccd2d9-a32a-4fc2-923d-f2c8c93e89d4.xml"}}, {"value": "2.0447E-05", "module": "A1-A3"}, {"value": "8.328E-08", "module": "A5"}, {"value": "7.72E-07", "module": "C2", "scenario": "S1"}, {"value": "6.798E-07", "module": "C2", "scenario": "S2"}, {"value": "8.098E-07", "module": "C3", "scenario": "S1"}, {"value": "0", "module": "C3", "scenario": "S2"}, {"value": "0", "module": "C4", "scenario": "S1"}, {"value": "4.315E-07", "module": "C4", "scenario": "S2"}, {"value": "-1.763E-06", "module": "D", "scenario": "S1"}, {"value": "-4.059E-07", "module": "D", "scenario": "S2"}]}}, {"referenceToLCIAMethodDataSet": {"shortDescription": [{"value": "Abiotic depletion potential for fossil resources (ADPF)", "lang": "en"}, {"value": "Potenzial für den abiotischen Abbau fossiler Brennstoffe (ADPF)", "lang": "de"}], "type": "LCIA method data set", "refObjectId": "b2ad6110-c78d-11e6-9d9d-cec0c932ce01", "uri": "../lciamethods/b2ad6110-c78d-11e6-9d9d-cec0c932ce01.xml"}, "other": {"anies": [{"name": "referenceToUnitGroupDataSet", "value": {"shortDescription": [{"value": "MJ", "lang": "en"}], "type": "unit group data set", "refObjectId": "93a60a57-a3c8-11da-a746-0800200c9a66", "uri": "../unitgroups/93a60a57-a3c8-11da-a746-0800200c9a66.xml"}}, {"value": "364.16", "module": "A1-A3"}, {"value": "0.498", "module": "A5"}, {"value": "4.323", "module": "C2", "scenario": "S1"}, {"value": "3.807", "module": "C2", "scenario": "S2"}, {"value": "7.391", "module": "C3", "scenario": "S1"}, {"value": "0", "module": "C3", "scenario": "S2"}, {"value": "0", "module": "C4", "scenario": "S1"}, {"value": "5.196", "module": "C4", "scenario": "S2"}, {"value": "-12.99", "module": "D", "scenario": "S1"}, {"value": "-2.867", "module": "D", "scenario": "S2"}]}}, {"referenceToLCIAMethodDataSet": {"shortDescription": [{"value": "Water use (WDP)", "lang": "en"}, {"value": "Wassernutzung (WDP)", "lang": "de"}], "type": "LCIA method data set", "refObjectId": "b2ad66ce-c78d-11e6-9d9d-cec0c932ce01", "uri": "../lciamethods/b2ad66ce-c78d-11e6-9d9d-cec0c932ce01.xml"}, "other": {"anies": [{"name": "referenceToUnitGroupDataSet", "value": {"shortDescription": [{"value": "m^(3) world eq deprived", "lang": "en"}], "type": "unit group data set", "refObjectId": "6ae2df01-888e-46c8-b17d-49fa3869b476", "uri": "../unitgroups/6ae2df01-888e-46c8-b17d-49fa3869b476.xml"}}, {"value": "0.79622", "module": "A1-A3"}, {"value": "0.002767", "module": "A5"}, {"value": "0.01316", "module": "C2", "scenario": "S1"}, {"value": "0.01159", "module": "C2", "scenario": "S2"}, {"value": "0.09527", "module": "C3", "scenario": "S1"}, {"value": "0", "module": "C3", "scenario": "S2"}, {"value": "0", "module": "C4", "scenario": "S1"}, {"value": "0.02433", "module": "C4", "scenario": "S2"}, {"value": "-0.1165", "module": "D", "scenario": "S1"}, {"value": "-0.05539", "module": "D", "scenario": "S2"}]}}, {"referenceToLCIAMethodDataSet": {"shortDescription": [{"value": "Incidence of disease due to PM emissions (PM)", "lang": "en"}, {"value": "Auftreten von Krankheiten aufgrund von Feinstaubemissionen (PM)", "lang": "de"}], "type": "LCIA method data set", "refObjectId": "b5c602c6-def3-11e6-bf01-fe55135034f3", "uri": "../lciamethods/b5c602c6-def3-11e6-bf01-fe55135034f3.xml"}, "other": {"anies": [{"name": "referenceToUnitGroupDataSet", "value": {"shortDescription": [{"value": "Disease incidence", "lang": "en"}], "type": "unit group data set", "refObjectId": "3883559b-648f-4afc-8ba2-0bd24f3affa3", "uri": "../unitgroups/3883559b-648f-4afc-8ba2-0bd24f3affa3.xml"}}, {"value": "4.3788E-07", "module": "A1-A3"}, {"value": "3.646E-09", "module": "A5"}, {"value": "2.291E-08", "module": "C2", "scenario": "S1"}, {"value": "2.017E-08", "module": "C2", "scenario": "S2"}, {"value": "1.167E-08", "module": "C3", "scenario": "S1"}, {"value": "0", "module": "C3", "scenario": "S2"}, {"value": "0", "module": "C4", "scenario": "S1"}, {"value": "3.111E-08", "module": "C4", "scenario": "S2"}, {"value": "-4.035E-08", "module": "D", "scenario": "S1"}, {"value": "-1.379E-08", "module": "D", "scenario": "S2"}]}}, {"referenceToLCIAMethodDataSet": {"shortDescription": [{"value": "Human exposure efficiency relative to U235 (IR)", "lang": "en"}, {"value": "Wirkung durch Exposition des Menschen mit U235 (IR)", "lang": "de"}], "type": "LCIA method data set", "refObjectId": "b5c632be-def3-11e6-bf01-fe55135034f3", "uri": "../lciamethods/b5c632be-def3-11e6-bf01-fe55135034f3.xml"}, "other": {"anies": [{"name": "referenceToUnitGroupDataSet", "value": {"shortDescription": [{"value": "kBq U235 eq", "lang": "en"}], "type": "unit group data set", "refObjectId": "456b05bf-1415-44a9-9993-02452f554c09", "uri": "../unitgroups/456b05bf-1415-44a9-9993-02452f554c09.xml"}}, {"value": "0.54808", "module": "A1-A3"}, {"value": "0.002232", "module": "A5"}, {"value": "0.01877", "module": "C2", "scenario": "S1"}, {"value": "0.01653", "module": "C2", "scenario": "S2"}, {"value": "0.06387", "module": "C3", "scenario": "S1"}, {"value": "0", "module": "C3", "scenario": "S2"}, {"value": "0", "module": "C4", "scenario": "S1"}, {"value": "0.02655", "module": "C4", "scenario": "S2"}, {"value": "-0.05914", "module": "D", "scenario": "S1"}, {"value": "-0.01341", "module": "D", "scenario": "S2"}]}}, {"referenceToLCIAMethodDataSet": {"shortDescription": [{"value": "Comparative toxic unit for ecosystems (ETP-fw)", "lang": "en"}, {"value": "Toxizitätsvergleichseinheit für Ökosysteme (ETP-fw)", "lang": "de"}], "type": "LCIA method data set", "refObjectId": "ee1082d1-b0f7-43ca-a1f0-21e2a4a74511", "uri": "../lciamethods/ee1082d1-b0f7-43ca-a1f0-21e2a4a74511.xml"}, "other": {"anies": [{"name": "referenceToUnitGroupDataSet", "value": {"shortDescription": [{"value": "CTUe", "lang": "en"}], "type": "unit group data set", "refObjectId": "aa959ded-f1eb-4efb-9c5c-2d60be36b3e6", "uri": "../unitgroups/aa959ded-f1eb-4efb-9c5c-2d60be36b3e6.xml"}}, {"value": "234.57", "module": "A1-A3"}, {"value": "0.4458", "module": "A5"}, {"value": "3.393", "module": "C2", "scenario": "S1"}, {"value": "2.988", "module": "C2", "scenario": "S2"}, {"value": "7.273", "module": "C3", "scenario": "S1"}, {"value": "0", "module": "C3", "scenario": "S2"}, {"value": "0", "module": "C4", "scenario": "S1"}, {"value": "2.985", "module": "C4", "scenario": "S2"}, {"value": "-68.49", "module": "D", "scenario": "S1"}, {"value": "-1.817", "module": "D", "scenario": "S2"}]}}, {"referenceToLCIAMethodDataSet": {"shortDescription": [{"value": "Comparative toxic unit for humans (carcinogenic) (HTP-c)", "lang": "en"}, {"value": "Toxizitätsvergleichseinheit für Menschen (krebserregend) (HTP-c)", "lang": "de"}], "type": "LCIA method data set", "refObjectId": "2299222a-bbd8-474f-9d4f-4dd1f18aea7c", "uri": "../lciamethods/2299222a-bbd8-474f-9d4f-4dd1f18aea7c.xml"}, "other": {"anies": [{"name": "referenceToUnitGroupDataSet", "value": {"shortDescription": [{"value": "CTUh", "lang": "en"}], "type": "unit group data set", "refObjectId": "d4c9523e-2d7e-49fd-8469-998f547d3a70", "uri": "../unitgroups/d4c9523e-2d7e-49fd-8469-998f547d3a70.xml"}}, {"value": "6.1119E-09", "module": "A1-A3"}, {"value": "1.076E-10", "module": "A5"}, {"value": "1.091E-10", "module": "C2", "scenario": "S1"}, {"value": "9.609E-11", "module": "C2", "scenario": "S2"}, {"value": "6.005E-10", "module": "C3", "scenario": "S1"}, {"value": "0", "module": "C3", "scenario": "S2"}, {"value": "0", "module": "C4", "scenario": "S1"}, {"value": "8.659E-11", "module": "C4", "scenario": "S2"}, {"value": "-2.148E-10", "module": "D", "scenario": "S1"}, {"value": "-7.561E-11", "module": "D", "scenario": "S2"}]}}, {"referenceToLCIAMethodDataSet": {"shortDescription": [{"value": "Comparative toxic unit for humans (noncarcinogenic) (HTP-nc)", "lang": "en"}, {"value": "Toxizitätsvergleichseinheit für Menschen (nicht krebserregend) (HTP-nc)", "lang": "de"}], "type": "LCIA method data set", "refObjectId": "3af763a5-b7a1-48c9-9cee-1f223481fcef", "uri": "../lciamethods/3af763a5-b7a1-48c9-9cee-1f223481fcef.xml"}, "other": {"anies": [{"name": "referenceToUnitGroupDataSet", "value": {"shortDescription": [{"value": "CTUh", "lang": "en"}], "type": "unit group data set", "refObjectId": "d4c9523e-2d7e-49fd-8469-998f547d3a70", "uri": "../unitgroups/d4c9523e-2d7e-49fd-8469-998f547d3a70.xml"}}, {"value": "1.423E-07", "module": "A1-A3"}, {"value": "6.584E-10", "module": "A5"}, {"value": "3.429E-09", "module": "C2", "scenario": "S1"}, {"value": "3.019E-09", "module": "C2", "scenario": "S2"}, {"value": "6.507E-09", "module": "C3", "scenario": "S1"}, {"value": "0", "module": "C3", "scenario": "S2"}, {"value": "0", "module": "C4", "scenario": "S1"}, {"value": "1.752E-09", "module": "C4", "scenario": "S2"}, {"value": "-5.532E-09", "module": "D", "scenario": "S1"}, {"value": "-1.775E-09", "module": "D", "scenario": "S2"}]}}, {"referenceToLCIAMethodDataSet": {"shortDescription": [{"value": "Soil quality index (SQP)", "lang": "en"}, {"value": "Bodenqualitätsindex (SQP)", "lang": "de"}], "type": "LCIA method data set", "refObjectId": "b2ad6890-c78d-11e6-9d9d-cec0c932ce01", "uri": "../lciamethods/b2ad6890-c78d-11e6-9d9d-cec0c932ce01.xml"}, "other": {"anies": [{"name": "referenceToUnitGroupDataSet", "value": {"shortDescription": [{"value": "SQP", "lang": "en"}], "type": "unit group data set", "refObjectId": "f130951c-e67f-4f7f-8dd4-665de3974e18", "uri": "../unitgroups/f130951c-e67f-4f7f-8dd4-665de3974e18.xml"}}, {"value": "455.205", "module": "A1-A3"}, {"value": "0.4919", "module": "A5"}, {"value": "3.013", "module": "C2", "scenario": "S1"}, {"value": "2.653", "module": "C2", "scenario": "S2"}, {"value": "1.606", "module": "C3", "scenario": "S1"}, {"value": "0", "module": "C3", "scenario": "S2"}, {"value": "0", "module": "C4", "scenario": "S1"}, {"value": "9.798", "module": "C4", "scenario": "S2"}, {"value": "-59.25", "module": "D", "scenario": "S1"}, {"value": "-57.92", "module": "D", "scenario": "S2"}]}}]}, "otherAttributes": {"{http://www.indata.network/EPD/2019}epd-version": "1.2"}, "version": "1.1", "locations": "../ILCDLocations.xml"}