{"processInformation": {"dataSetInformation": {"UUID": "6a497eaa-2a18-4cc6-a023-64d1779a4f19", "name": {"baseName": [{"value": "Sarnafil TG 76 FSA", "lang": "de"}, {"value": "Sarnafil TG 76 FSA", "lang": "en"}], "functionalUnitFlowProperties": [{"lang": "de"}]}, "classificationInformation": {"classification": [{"class": [{"value": "Kunststoffe", "level": 0, "classId": "6"}, {"value": "Dachbahnen", "level": 1, "classId": "6.3"}, {"value": "Elastomer-Dachbahnen", "level": 2, "classId": "6.3.03"}], "name": "OEKOBAU.DAT"}, {"class": [{"value": "02 Bauprodukte", "level": 0}, {"value": "Abdichtungen", "level": 1}, {"value": "Dach- und Dichtungsbahnsysteme aus Kunststoffen und Elastomeren", "level": 2}], "name": "IBUCategories"}]}, "generalComment": [{"value": "Sarnafil® TG 76 FSA Kunststoffabdichtungsbahnen bestehen aus flexiblen Polyolefinen (FPO) und werden zustzlich mit UV-Lichtschutzmittel, Flammschutzmittel und einer unterseitigen Kaschierung mit Glas/Polyestermischvlies mit integrierter Selbstklebeschicht und \"Release Liner\" ausgerstet. Die sind jeweils mit einer inne liegenden Einlage aus Glasvlies und Glasgitter versehen. Die unterseitige Glaspolyestermischvlieskaschierung dient als Haftbrcke und Ausgleichslage fr die direkte flchige Verklebung mit der Selbstklebeschicht auf Wrmedmmung aus expandiertem Polystyrol (EPS) Mineralwolle und Polyurethan (PU).", "lang": "de"}, {"value": "Sarnafil® TG 76 FSA polymeric waterproofing membrane is made of flexible polyolefin (FPO) and is treated with flame retardant and stabilizers against UV radiation and backed with a glass-polyester nonwoven mat (felt) with an integral adhesive coating and release liner. An inlay composed of glass felt and glass mesh is encapsulated within the sheet. The glass-polyester felt backing serves as a bonding and levelling layer for fully adhered application by means of the adhesive coating over insulation layers consisting of expanded polystyrene (EPS) or polyurethane (PU).", "lang": "en"}]}, "quantitativeReference": {"referenceToReferenceFlow": [0]}, "time": {"referenceYear": 2023, "dataSetValidUntil": 2028, "other": {"anies": [{"name": "publicationDateOfEPD", "value": 1683158400000}]}}, "geography": {"locationOfOperationSupplyOrProduction": {"location": "CH"}}, "technology": {"technologyDescriptionAndIncludedProcesses": [{"value": "Der Herstellungsprozess der Sarnafil® TG 76 FSA Kunststoffabdichtungsbahnen verläuft auf eigens entwickelten Produktionsanlagen in folgenden Schritten: Aufschmelzen der Kunststoffkomponenten sowie ihrer Additive in ExtrudernDispergieren der aufgeschmolzenen MaterialienAufbringen der Schichten auf den Träger bzw. die Armierung, so dass eine homogene Einbettung erfolgtAufbringen der unterseitigen VlieskaschierungAufbringen der Selbstklebeschicht Kühlen der KunststoffabdichtungsbahnAufwickeln der Kunststoffabdichtungsbahn auf Rollenkerne aus AltpapierkartonageVerpacken der einzelnen Rollen mit einer PE-Folie Das Werk Sarnen verfügt seit 1993 über ein zertifizier-tes Qualitätsmanagementsystem nach \"ISO 9001\". \nDeklarierte Einheit: \nDiese Deklaration bezieht sich auf 1 m2 Sarnafil® TG 76 FSA-Kunststoffabdichtungsbahn mit der Dicke 1,8 mm.\n\nFr andere Dicken wird eine Formel zur eigenstndigen Berechnung der Werte angegeben.", "lang": "de"}, {"value": "- \nDeclared unit: \nThis declaration applies to 1 m2 of installed Sarnafil® TG 76 FSA polymeric waterproofing membrane, thickness 1,8 mm.\n\nA formula is given for independent calculation of the values for other thicknesses.", "lang": "en"}], "technologicalApplicability": [{"value": "Sarnafil® TG 76 FSA Kunststoffabdichtungsbahnen dienen hauptschlich der Abdichtung von Flachdchern. Die Dachbahnen knnen auf Dchern ohne Auflast flchig verklebt werden. Die Verlegung auf Dchern mit Kiesauflast und Begrnung ist ebenfalls mglich.", "lang": "de"}, {"value": "Sarnafil® TG 76 FSA polymeric waterproofing membrane is used chiefly to seal flat roofs. The roofing sheets can be fully adhered to roofs without ballast. Application on roofs with gravel ballast or in green roof systems is also possible.", "lang": "en"}]}}, "modellingAndValidation": {"LCIMethodAndAllocation": {"typeOfDataSet": "EPD", "referenceToLCAMethodDetails": [{"shortDescription": [{"value": "Dach- und Dichtungsbahnsysteme aus Kunststoffen und Elastomeren.pdf", "lang": "de"}], "type": "source data set", "refObjectId": "2ae4968b-d745-4e38-a303-973f7cd8e52b"}], "other": {"anies": [{"name": "subType", "value": "average dataset"}]}}, "dataSourcesTreatmentAndRepresentativeness": {"referenceToDataSource": [{"shortDescription": [{"value": "GaBi Database (all versions)", "lang": "de"}], "type": "source data set", "refObjectId": "28d74cc0-db8b-4d7e-bc44-5f6d56ce0c4a"}, {"shortDescription": [{"value": "GaBi Database Edition 2022, CUP 2022.01", "lang": "de"}], "type": "source data set", "refObjectId": "86f664e2-7dab-4722-aad7-4c5206a4123b"}], "useAdviceForDataSet": [{"value": "Gültigkeitsbereich: \nDieses Dokument bezieht sich auf die von der Sika AG in CH-6060 Sarnen (Schweiz) hergestellten Sarnafil® TG 76 FSA Kunststoffabdichtungsbahnen.\n\nDie kobilanzdaten wurden auf Basis der Produktionsdaten aus dem Jahr 2021 von der Sika Technology AG erfasst. \nSystemgrenze: \nTyp der EPD: Wiege bis Werkstor - mit Optionen.\n\nDie Systemgrenze der EPD folgt dem modularen Aufbau gem EN 15804. In der kobilanz werden die folgenden Module bercksichtigt:\nA1–A3: Herstellung der Vorprodukte, Verpackung sowie Hilfsstoffe, Transport zum Werk, Produktion inkl. Energiebereitstellung und Abfallbehandlung \nA4: Transport zur Baustelle \nA5: Einbau ins Gebude (Schweienergie, Entsorgung von Verpackung und Verschnitt der Dachbahn)\nC1: Rckbau und Abriss \nC2: Transport zur Abfallbewirtschaftung \nC3: Abfallbewirtschaftung zur Wiederverwendung, Rckgewinnung und/oder zum Recycling \nC4: Beseitigung (Abfallverbrennungsprozess) \nD: Wiederverwendungs-, Rckgewinnungs- und/oder Recyclingpotentiale (Gutschriften aus der Verbrennung und Rckgewinnung der Verpackungsmaterialien)", "lang": "de"}, {"value": "Scope: \nThis document applies to Sarnafil® TG 76 FSA polymeric waterproofing membrane manufactured by Sika AG in CH-6060 Sarnen (Switzerland).\n\nThe EPD has been calculated based on 2021 production data collected by Sika Technology AG. \nSystem boundary: \nType of EPD: Cradle to gate with options\n\nThe system boundaries of the EPD follow the modular buildup system as described by EN 15804. The LCA takes into account the following modules:\n\nA1-A3: Production of the intermediate products, packaging and ancillary materials, transport to the plant, production including energy supply and waste handling\nA4: Transport to the building site\nA5: Installation into the building (hot-air welding energy, disposal of packaging and waterproofing membrane scraps)\n\nC1: Deconstruction and demolition\nC2: Transport to waste-processing facility\nC3: Waste processing by reuse, recovery, and/or recycling\nC4: Disposal (incineration)\nD: Reuse, recovery and/or recycling potential (benefits from thermal energy recovery and recovery of packaging materials)", "lang": "en"}], "other": {"anies": [{"name": "referenceToOriginalEPD", "value": {"shortDescription": {"value": "Sarnafil TG 76 FSA.pdf", "defaultValue": "Sarnafil TG 76 FSA.pdf", "lstrings": [{"lang": "de", "value": "Sarnafil TG 76 FSA.pdf"}]}, "type": "source data set", "uuid": {"uuid": "2b0a063f-cf0c-4746-9c21-780fc6367f6f"}, "refObjectId": "2b0a063f-cf0c-4746-9c21-780fc6367f6f", "resourceURLs": ["https://oekobaudat.de/OEKOBAU.DAT/resource/sources/2b0a063f-cf0c-4746-9c21-780fc6367f6f/Sarnafil_TG_76_FSA_23273.pdf?version=00.04.000"]}}]}}, "validation": {"review": [{"referenceToNameOfReviewerAndInstitution": [{"shortDescription": [{"value": "Institut Bauen und Umwelt e. V.", "lang": "de"}], "type": "contact data set", "refObjectId": "d111dbec-b024-4be5-86c5-752d6eb2cf95", "uri": "../contacts/d111dbec-b024-4be5-86c5-752d6eb2cf95.xml"}], "type": "Accredited third party review"}]}, "complianceDeclarations": {"compliance": [{"referenceToComplianceSystem": {"shortDescription": [{"value": "DIN EN 15804+A2", "lang": "de"}], "type": "source data set", "refObjectId": "c0016b33-8cf7-415c-ac6e-deba0d21440d", "uri": "../sources/c0016b33-8cf7-415c-ac6e-deba0d21440d.xml"}}, {"referenceToComplianceSystem": {"shortDescription": [{"value": "ISO 14025", "lang": "de"}], "type": "source data set", "refObjectId": "4f2eb655-6e44-4874-a95a-e28f5442cd4d", "uri": "../sources/4f2eb655-6e44-4874-a95a-e28f5442cd4d.xml"}}]}}, "administrativeInformation": {"commissionerAndGoal": {"referenceToCommissioner": [{"shortDescription": [{"value": "Sika Deutschland GmbH", "lang": "de"}], "type": "contact data set", "refObjectId": "3d99c862-ca4d-4bff-9241-8a83668bd310", "uri": "../contacts/3d99c862-ca4d-4bff-9241-8a83668bd310.xml"}]}, "dataGenerator": {"referenceToPersonOrEntityGeneratingTheDataSet": [{"shortDescription": [{"value": "Sika Technology AG", "lang": "de"}], "type": "contact data set", "refObjectId": "e6e310ee-d48d-41ec-b502-68ec650bae28", "uri": "../contacts/e6e310ee-d48d-41ec-b502-68ec650bae28.xml"}]}, "dataEntryBy": {"timeStamp": 1683158400000, "referenceToDataSetFormat": [{"shortDescription": [{"value": "ILCD Format", "lang": "de"}], "type": "source data set", "refObjectId": "a97a0155-0234-4b87-b4ce-a45da52f2a40", "uri": "../sources/a97a0155-0234-4b87-b4ce-a45da52f2a40.xml"}, {"shortDescription": [{"value": "EPD-Datenformaterweiterungen v1.2", "lang": "de"}, {"value": "EPD Data Format Extensions v1.2", "lang": "en"}], "type": "source data set", "refObjectId": "a29449fd-aa2f-4de8-b5d7-4b06b43c6fde", "uri": "../sources/a29449fd-aa2f-4de8-b5d7-4b06b43c6fde.xml"}]}, "publicationAndOwnership": {"dataSetVersion": "00.07.000", "referenceToRegistrationAuthority": {"shortDescription": [{"value": "Institut Bauen und Umwelt e. V.", "lang": "de"}], "type": "contact data set", "refObjectId": "d111dbec-b024-4be5-86c5-752d6eb2cf95", "uri": "../contacts/d111dbec-b024-4be5-86c5-752d6eb2cf95.xml"}, "registrationNumber": "EPD-SIK-20220222-IBA2-DE", "referenceToOwnershipOfDataSet": {"shortDescription": [{"value": "Sika Deutschland GmbH", "lang": "de"}], "type": "contact data set", "refObjectId": "3d99c862-ca4d-4bff-9241-8a83668bd310", "uri": "../contacts/3d99c862-ca4d-4bff-9241-8a83668bd310.xml"}, "copyright": true, "licenseType": "Free of charge for all users and uses", "accessRestrictions": [{"value": "None", "lang": "en"}], "other": {"anies": [{"name": "referenceToPublisher", "value": {"shortDescription": [{"value": "Institut Bauen und Umwelt e. V.", "lang": "de"}], "type": "contact data set", "refObjectId": "d111dbec-b024-4be5-86c5-752d6eb2cf95", "uri": "../contacts/d111dbec-b024-4be5-86c5-752d6eb2cf95.xml"}}]}}}, "exchanges": {"exchange": [{"dataSetInternalID": 0, "referenceToFlowDataSet": {"shortDescription": [{"value": "Dachbahn (Dachbahn)", "lang": "de"}], "type": "flow data set", "refObjectId": "f094ac99-27f0-981a-0f7f-4e5c4b6eb216", "uri": "../flows/f094ac99-27f0-981a-0f7f-4e5c4b6eb216.xml"}, "meanAmount": 1.0, "referencesToDataSource": {}, "referenceFlow": true, "resolvedFlowVersion": "00.05.000", "resultingflowAmount": 1.0, "flowProperties": [{"name": [{"lang": "en", "value": "Area"}, {"lang": "de", "value": "Fläche"}], "uuid": "93a60a56-a3c8-19da-a746-0800200c9a66", "referenceFlowProperty": true, "meanValue": 1.0, "referenceUnit": "qm", "unitGroupUUID": "c20a03d7-bd90-4569-bc94-66cfd364dfc8"}], "materialProperties": [{"name": "layer thickness", "value": "0.0018", "unit": "m", "unitDescription": "meters"}, {"name": "grammage", "value": "2.3", "unit": "kg/m^2", "unitDescription": "kilograms per square meter"}, {"name": "conversion factor to 1 kg", "value": "0.43", "unit": "-", "unitDescription": "Without unit"}], "typeOfFlow": "Product flow", "classification": {"classHierarchy": "Kunststoffe / Dachbahnen / Elastomer-Dachbahnen", "name": "OEKOBAU.DAT"}}, {"dataSetInternalID": 1, "referenceToFlowDataSet": {"shortDescription": [{"value": "Erneuerbare Primärenergie als Energieträger (PERE)", "lang": "de"}, {"value": "Renewable primary energy as energy carrier (PERE)", "lang": "en"}], "type": "flow data set", "refObjectId": "20f32be5-0398-4288-9b6d-accddd195317", "uri": "../flows/20f32be5-0398-4288-9b6d-accddd195317.xml"}, "exchange direction": "INPUT", "other": {"anies": [{"name": "referenceToUnitGroupDataSet", "value": {"shortDescription": [{"value": "MJ", "lang": "de"}], "type": "unit group data set", "refObjectId": "93a60a57-a3c8-11da-a746-0800200c9a66", "uri": "../unitgroups/93a60a57-a3c8-11da-a746-0800200c9a66.xml"}}, {"value": "8.37373333333333", "module": "A1-A3"}, {"value": "0.0840952380952381", "module": "A4"}, {"value": "0.206280952380952", "module": "A5"}, {"module": "C1"}, {"value": "0.00691", "module": "C2"}, {"value": "0.207", "module": "C3"}, {"value": "0", "module": "C4"}, {"value": "-25.2", "module": "D"}]}, "resolvedFlowVersion": "38.00.000", "flowProperties": [], "typeOfFlow": "Other flow", "classification": {"classHierarchy": "Quantities", "name": "GaBiCategories"}}, {"dataSetInternalID": 2, "referenceToFlowDataSet": {"shortDescription": [{"value": "Erneuerbare Primärenergie zur stofflichen Nutzung (PERM)", "lang": "de"}, {"value": "Renewable primary energy resources as material utilization (PERM)", "lang": "en"}], "type": "flow data set", "refObjectId": "fb3ec0de-548d-4508-aea5-00b73bf6f702", "uri": "../flows/fb3ec0de-548d-4508-aea5-00b73bf6f702.xml"}, "exchange direction": "INPUT", "other": {"anies": [{"name": "referenceToUnitGroupDataSet", "value": {"shortDescription": [{"value": "MJ", "lang": "de"}], "type": "unit group data set", "refObjectId": "93a60a57-a3c8-11da-a746-0800200c9a66", "uri": "../unitgroups/93a60a57-a3c8-11da-a746-0800200c9a66.xml"}}, {"value": "1.53102857142857", "module": "A1-A3"}, {"value": "0", "module": "A4"}, {"value": "-0.0765514285714286", "module": "A5"}, {"module": "C1"}, {"value": "0", "module": "C2"}, {"value": "0", "module": "C3"}, {"value": "0", "module": "C4"}, {"value": "0", "module": "D"}]}, "resolvedFlowVersion": "38.00.000", "flowProperties": [], "typeOfFlow": "Other flow", "classification": {"classHierarchy": "Quantities", "name": "GaBiCategories"}}, {"dataSetInternalID": 3, "referenceToFlowDataSet": {"shortDescription": [{"value": "Total erneuerbare Primärenergie (PERT)", "lang": "de"}, {"value": "Total use of renewable primary energy resources (PERT)", "lang": "en"}], "type": "flow data set", "refObjectId": "53f97275-fa8a-4cdd-9024-65936002acd0", "uri": "../flows/53f97275-fa8a-4cdd-9024-65936002acd0.xml"}, "exchange direction": "INPUT", "other": {"anies": [{"name": "referenceToUnitGroupDataSet", "value": {"shortDescription": [{"value": "MJ", "lang": "de"}], "type": "unit group data set", "refObjectId": "93a60a57-a3c8-11da-a746-0800200c9a66", "uri": "../unitgroups/93a60a57-a3c8-11da-a746-0800200c9a66.xml"}}, {"value": "9.90476190476191", "module": "A1-A3"}, {"value": "0.0840952380952381", "module": "A4"}, {"value": "0.129729523809524", "module": "A5"}, {"module": "C1"}, {"value": "0.00691", "module": "C2"}, {"value": "0.207", "module": "C3"}, {"value": "0", "module": "C4"}, {"value": "-25.2", "module": "D"}]}, "resolvedFlowVersion": "38.00.000", "flowProperties": [], "typeOfFlow": "Other flow", "classification": {"classHierarchy": "Quantities / Environmental quantities / EPD EN 15804 / LCI indicators", "name": "GaBiCategories"}}, {"dataSetInternalID": 4, "referenceToFlowDataSet": {"shortDescription": [{"value": "Nicht-erneuerbare Primärenergie als Energieträger (PENRE)", "lang": "de"}, {"value": "Non renewable primary energy as energy carrier (PENRE)", "lang": "en"}], "type": "flow data set", "refObjectId": "ac857178-2b45-46ec-892a-a9a4332f0372", "uri": "../flows/ac857178-2b45-46ec-892a-a9a4332f0372.xml"}, "exchange direction": "INPUT", "other": {"anies": [{"name": "referenceToUnitGroupDataSet", "value": {"shortDescription": [{"value": "MJ", "lang": "de"}], "type": "unit group data set", "refObjectId": "93a60a57-a3c8-11da-a746-0800200c9a66", "uri": "../unitgroups/93a60a57-a3c8-11da-a746-0800200c9a66.xml"}}, {"value": "-24.0188266666667", "module": "A1-A3"}, {"value": "1.48571428571429", "module": "A4"}, {"value": "-0.253094476190475", "module": "A5"}, {"module": "C1"}, {"value": "0", "module": "C2"}, {"value": "98.2615330285714", "module": "C3"}, {"value": "0", "module": "C4"}, {"value": "-61.1", "module": "D"}]}, "resolvedFlowVersion": "38.00.000", "flowProperties": [], "typeOfFlow": "Other flow", "classification": {"classHierarchy": "Quantities", "name": "GaBiCategories"}}, {"dataSetInternalID": 5, "referenceToFlowDataSet": {"shortDescription": [{"value": "Nicht-erneuerbare Primärenergie zur stofflichen Nutzung (PENRM)", "lang": "de"}, {"value": "Non renewable primary energy as material utilization (PENRM)", "lang": "en"}], "type": "flow data set", "refObjectId": "1421caa0-679d-4bf4-b282-0eb850ccae27", "uri": "../flows/1421caa0-679d-4bf4-b282-0eb850ccae27.xml"}, "exchange direction": "INPUT", "other": {"anies": [{"name": "referenceToUnitGroupDataSet", "value": {"shortDescription": [{"value": "MJ", "lang": "de"}], "type": "unit group data set", "refObjectId": "93a60a57-a3c8-11da-a746-0800200c9a66", "uri": "../unitgroups/93a60a57-a3c8-11da-a746-0800200c9a66.xml"}}, {"value": "95.6378742857143", "module": "A1-A3"}, {"value": "0", "module": "A4"}, {"value": "4.04733257142857", "module": "A5"}, {"module": "C1"}, {"value": "0", "module": "C2"}, {"value": "-97.3825330285714", "module": "C3"}, {"value": "0", "module": "C4"}, {"value": "0", "module": "D"}]}, "resolvedFlowVersion": "38.00.000", "flowProperties": [], "typeOfFlow": "Other flow", "classification": {"classHierarchy": "Quantities", "name": "GaBiCategories"}}, {"dataSetInternalID": 6, "referenceToFlowDataSet": {"shortDescription": [{"value": "Total nicht erneuerbare Primärenergie (PENRT)", "lang": "de"}, {"value": "Total use of non renewable primary energy resources (PENRT)", "lang": "en"}], "type": "flow data set", "refObjectId": "06159210-646b-4c8d-8583-da9b3b95a6c1", "uri": "../flows/06159210-646b-4c8d-8583-da9b3b95a6c1.xml"}, "exchange direction": "INPUT", "other": {"anies": [{"name": "referenceToUnitGroupDataSet", "value": {"shortDescription": [{"value": "MJ", "lang": "de"}], "type": "unit group data set", "refObjectId": "93a60a57-a3c8-11da-a746-0800200c9a66", "uri": "../unitgroups/93a60a57-a3c8-11da-a746-0800200c9a66.xml"}}, {"value": "71.6190476190476", "module": "A1-A3"}, {"value": "1.48571428571429", "module": "A4"}, {"value": "3.7942380952381", "module": "A5"}, {"module": "C1"}, {"value": "0.122", "module": "C2"}, {"value": "0.879", "module": "C3"}, {"value": "0", "module": "C4"}, {"value": "-61.1", "module": "D"}]}, "resolvedFlowVersion": "38.00.000", "flowProperties": [], "typeOfFlow": "Other flow", "classification": {"classHierarchy": "Quantities / Environmental quantities / EPD EN 15804 / LCI indicators", "name": "GaBiCategories"}}, {"dataSetInternalID": 7, "referenceToFlowDataSet": {"shortDescription": [{"value": "Einsatz von Sekundärstoffen (SM)", "lang": "de"}, {"value": "Use of secondary material (SM)", "lang": "en"}], "type": "flow data set", "refObjectId": "c6a1f35f-2d09-4f54-8dfb-97e502e1ce92", "uri": "../flows/c6a1f35f-2d09-4f54-8dfb-97e502e1ce92.xml"}, "exchange direction": "INPUT", "other": {"anies": [{"name": "referenceToUnitGroupDataSet", "value": {"shortDescription": [{"value": "kg", "lang": "de"}], "type": "unit group data set", "refObjectId": "ad38d542-3fe9-439d-9b95-2f5f7752acaf", "uri": "../unitgroups/ad38d542-3fe9-439d-9b95-2f5f7752acaf.xml"}}, {"value": "0.0663809523809524", "module": "A1-A3"}, {"value": "0", "module": "A4"}, {"value": "0.00331904761904762", "module": "A5"}, {"module": "C1"}, {"value": "0", "module": "C2"}, {"value": "0", "module": "C3"}, {"value": "0", "module": "C4"}, {"value": "-0.0878", "module": "D"}]}, "resolvedFlowVersion": "38.00.000", "flowProperties": [], "typeOfFlow": "Other flow", "classification": {"classHierarchy": "Quantities / Environmental quantities / EPD EN 15804 / LCI indicators", "name": "GaBiCategories"}}, {"dataSetInternalID": 8, "referenceToFlowDataSet": {"shortDescription": [{"value": "Erneuerbare Sekundärbrennstoffe (RSF)", "lang": "de"}, {"value": "Use of renewable secondary fuels (RSF)", "lang": "en"}], "type": "flow data set", "refObjectId": "64333088-a55f-4aa2-9a31-c10b07816787", "uri": "../flows/64333088-a55f-4aa2-9a31-c10b07816787.xml"}, "exchange direction": "INPUT", "other": {"anies": [{"name": "referenceToUnitGroupDataSet", "value": {"shortDescription": [{"value": "MJ", "lang": "de"}], "type": "unit group data set", "refObjectId": "93a60a57-a3c8-11da-a746-0800200c9a66", "uri": "../unitgroups/93a60a57-a3c8-11da-a746-0800200c9a66.xml"}}, {"value": "0", "module": "A1-A3"}, {"value": "0", "module": "A4"}, {"value": "0", "module": "A5"}, {"module": "C1"}, {"value": "0", "module": "C2"}, {"value": "0", "module": "C3"}, {"value": "0", "module": "C4"}, {"value": "0", "module": "D"}]}, "resolvedFlowVersion": "38.00.000", "flowProperties": [], "typeOfFlow": "Other flow", "classification": {"classHierarchy": "Quantities / Environmental quantities / EPD EN 15804 / LCI indicators", "name": "GaBiCategories"}}, {"dataSetInternalID": 9, "referenceToFlowDataSet": {"shortDescription": [{"value": "Nicht erneuerbare Sekundärbrennstoffe (NRSF)", "lang": "de"}, {"value": "Use of non renewable secondary fuels (NRSF)", "lang": "en"}], "type": "flow data set", "refObjectId": "89def144-d39a-4287-b86f-efde453ddcb2", "uri": "../flows/89def144-d39a-4287-b86f-efde453ddcb2.xml"}, "exchange direction": "INPUT", "other": {"anies": [{"name": "referenceToUnitGroupDataSet", "value": {"shortDescription": [{"value": "MJ", "lang": "de"}], "type": "unit group data set", "refObjectId": "93a60a57-a3c8-11da-a746-0800200c9a66", "uri": "../unitgroups/93a60a57-a3c8-11da-a746-0800200c9a66.xml"}}, {"value": "0", "module": "A1-A3"}, {"value": "0", "module": "A4"}, {"value": "0", "module": "A5"}, {"module": "C1"}, {"value": "0", "module": "C2"}, {"value": "0", "module": "C3"}, {"value": "0", "module": "C4"}, {"value": "0", "module": "D"}]}, "resolvedFlowVersion": "38.00.000", "flowProperties": [], "typeOfFlow": "Other flow", "classification": {"classHierarchy": "Quantities / Environmental quantities / EPD EN 15804 / LCI indicators", "name": "GaBiCategories"}}, {"dataSetInternalID": 10, "referenceToFlowDataSet": {"shortDescription": [{"value": "Einsatz von Süßwasserressourcen (FW)", "lang": "de"}, {"value": "Use of net fresh water (FW)", "lang": "en"}], "type": "flow data set", "refObjectId": "3cf952c8-f3a4-461d-8c96-96456ca62246", "uri": "../flows/3cf952c8-f3a4-461d-8c96-96456ca62246.xml"}, "exchange direction": "INPUT", "other": {"anies": [{"name": "referenceToUnitGroupDataSet", "value": {"shortDescription": [{"value": "m^3", "lang": "de"}], "type": "unit group data set", "refObjectId": "cd950537-0a98-4044-9ba7-9f9a68d0a504", "uri": "../unitgroups/cd950537-0a98-4044-9ba7-9f9a68d0a504.xml"}}, {"value": "0.0448571428571429", "module": "A1-A3"}, {"value": "9.51428571428571E-05", "module": "A4"}, {"value": "0.00276361428571429", "module": "A5"}, {"module": "C1"}, {"value": "7.82E-06", "module": "C2"}, {"value": "0.0163", "module": "C3"}, {"value": "0", "module": "C4"}, {"value": "-0.01", "module": "D"}]}, "resolvedFlowVersion": "38.00.000", "flowProperties": [], "typeOfFlow": "Other flow", "classification": {"classHierarchy": "Quantities / Environmental quantities / EPD EN 15804 / LCI indicators", "name": "GaBiCategories"}}, {"dataSetInternalID": 11, "referenceToFlowDataSet": {"shortDescription": [{"value": "Gefährlicher Abfall zur Deponie (HWD)", "lang": "de"}, {"value": "Hazardous waste disposed (HWD)", "lang": "en"}], "type": "flow data set", "refObjectId": "430f9e0f-59b2-46a0-8e0d-55e0e84948fc", "uri": "../flows/430f9e0f-59b2-46a0-8e0d-55e0e84948fc.xml"}, "exchange direction": "OUTPUT", "other": {"anies": [{"name": "referenceToUnitGroupDataSet", "value": {"shortDescription": [{"value": "kg", "lang": "de"}], "type": "unit group data set", "refObjectId": "ad38d542-3fe9-439d-9b95-2f5f7752acaf", "uri": "../unitgroups/ad38d542-3fe9-439d-9b95-2f5f7752acaf.xml"}}, {"value": "1.66666666666667E-08", "module": "A1-A3"}, {"value": "7.1047619047619E-12", "module": "A4"}, {"value": "8.47088571428571E-10", "module": "A5"}, {"module": "C1"}, {"value": "5.84E-13", "module": "C2"}, {"value": "8.27E-11", "module": "C3"}, {"value": "0", "module": "C4"}, {"value": "-8.79E-09", "module": "D"}]}, "resolvedFlowVersion": "38.00.000", "flowProperties": [], "typeOfFlow": "Other flow", "classification": {"classHierarchy": "Quantities / Environmental quantities / EPD EN 15804 / LCI indicators", "name": "GaBiCategories"}}, {"dataSetInternalID": 12, "referenceToFlowDataSet": {"shortDescription": [{"value": "Entsorgter nicht gefährlicher Abfall (NHWD)", "lang": "de"}, {"value": "Non hazardous waste disposed (NHWD)", "lang": "en"}], "type": "flow data set", "refObjectId": "b29ef66b-e286-4afa-949f-62f1a7b4d7fa", "uri": "../flows/b29ef66b-e286-4afa-949f-62f1a7b4d7fa.xml"}, "exchange direction": "OUTPUT", "other": {"anies": [{"name": "referenceToUnitGroupDataSet", "value": {"shortDescription": [{"value": "kg", "lang": "de"}], "type": "unit group data set", "refObjectId": "ad38d542-3fe9-439d-9b95-2f5f7752acaf", "uri": "../unitgroups/ad38d542-3fe9-439d-9b95-2f5f7752acaf.xml"}}, {"value": "0.417142857142857", "module": "A1-A3"}, {"value": "0.000212380952380952", "module": "A4"}, {"value": "0.0228577619047619", "module": "A5"}, {"module": "C1"}, {"value": "1.75E-05", "module": "C2"}, {"value": "0.0299", "module": "C3"}, {"value": "0", "module": "C4"}, {"value": "-0.0374", "module": "D"}]}, "resolvedFlowVersion": "38.00.000", "flowProperties": [], "typeOfFlow": "Other flow", "classification": {"classHierarchy": "Quantities / Environmental quantities / EPD EN 15804 / LCI indicators", "name": "GaBiCategories"}}, {"dataSetInternalID": 13, "referenceToFlowDataSet": {"shortDescription": [{"value": "Entsorgter radioaktiver Abfall (RWD)", "lang": "de"}, {"value": "Radioactive waste disposed (RWD)", "lang": "en"}], "type": "flow data set", "refObjectId": "3449546e-52ad-4b39-b809-9fb77cea8ff6", "uri": "../flows/3449546e-52ad-4b39-b809-9fb77cea8ff6.xml"}, "exchange direction": "OUTPUT", "other": {"anies": [{"name": "referenceToUnitGroupDataSet", "value": {"shortDescription": [{"value": "kg", "lang": "de"}], "type": "unit group data set", "refObjectId": "ad38d542-3fe9-439d-9b95-2f5f7752acaf", "uri": "../unitgroups/ad38d542-3fe9-439d-9b95-2f5f7752acaf.xml"}}, {"value": "0.00166666666666667", "module": "A1-A3"}, {"value": "1.82857142857143E-06", "module": "A4"}, {"value": "9.39247619047619E-05", "module": "A5"}, {"module": "C1"}, {"value": "1.5E-07", "module": "C2"}, {"value": "5.32E-05", "module": "C3"}, {"value": "0", "module": "C4"}, {"value": "-0.0026", "module": "D"}]}, "resolvedFlowVersion": "38.00.000", "flowProperties": [], "typeOfFlow": "Other flow", "classification": {"classHierarchy": "Quantities / Environmental quantities / EPD EN 15804 / LCI indicators", "name": "GaBiCategories"}}, {"dataSetInternalID": 14, "referenceToFlowDataSet": {"shortDescription": [{"value": "Komponenten für die Wiederverwendung (CRU)", "lang": "de"}, {"value": "Components for re-use (CRU)", "lang": "en"}], "type": "flow data set", "refObjectId": "a2b32f97-3fc7-4af2-b209-525bc6426f33", "uri": "../flows/a2b32f97-3fc7-4af2-b209-525bc6426f33.xml"}, "exchange direction": "OUTPUT", "other": {"anies": [{"name": "referenceToUnitGroupDataSet", "value": {"shortDescription": [{"value": "kg", "lang": "de"}], "type": "unit group data set", "refObjectId": "ad38d542-3fe9-439d-9b95-2f5f7752acaf", "uri": "../unitgroups/ad38d542-3fe9-439d-9b95-2f5f7752acaf.xml"}}, {"value": "0", "module": "A1-A3"}, {"value": "0", "module": "A4"}, {"value": "0", "module": "A5"}, {"module": "C1"}, {"value": "0", "module": "C2"}, {"value": "0", "module": "C3"}, {"value": "0", "module": "C4"}, {"value": "0", "module": "D"}]}, "resolvedFlowVersion": "38.00.000", "flowProperties": [], "typeOfFlow": "Other flow", "classification": {"classHierarchy": "Quantities / Environmental quantities / EPD EN 15804 / LCI indicators", "name": "GaBiCategories"}}, {"dataSetInternalID": 15, "referenceToFlowDataSet": {"shortDescription": [{"value": "Stoffe zum Recycling (MFR)", "lang": "de"}, {"value": "Materials for recycling (MFR)", "lang": "en"}], "type": "flow data set", "refObjectId": "d7fe48a5-4103-49c8-9aae-b0b5dfdbd6ae", "uri": "../flows/d7fe48a5-4103-49c8-9aae-b0b5dfdbd6ae.xml"}, "exchange direction": "OUTPUT", "other": {"anies": [{"name": "referenceToUnitGroupDataSet", "value": {"shortDescription": [{"value": "kg", "lang": "de"}], "type": "unit group data set", "refObjectId": "ad38d542-3fe9-439d-9b95-2f5f7752acaf", "uri": "../unitgroups/ad38d542-3fe9-439d-9b95-2f5f7752acaf.xml"}}, {"value": "0", "module": "A1-A3"}, {"value": "0", "module": "A4"}, {"value": "0", "module": "A5"}, {"module": "C1"}, {"value": "0", "module": "C2"}, {"value": "0", "module": "C3"}, {"value": "0", "module": "C4"}, {"value": "0", "module": "D"}]}, "resolvedFlowVersion": "38.00.000", "flowProperties": [], "typeOfFlow": "Other flow", "classification": {"classHierarchy": "Quantities / Environmental quantities / EPD EN 15804 / LCI indicators", "name": "GaBiCategories"}}, {"dataSetInternalID": 16, "referenceToFlowDataSet": {"shortDescription": [{"value": "Stoffe für die Energierückgewinnung (MER)", "lang": "de"}, {"value": "Materials for energy recovery (MER)", "lang": "en"}], "type": "flow data set", "refObjectId": "59a9181c-3aaf-46ee-8b13-2b3723b6e447", "uri": "../flows/59a9181c-3aaf-46ee-8b13-2b3723b6e447.xml"}, "exchange direction": "OUTPUT", "other": {"anies": [{"name": "referenceToUnitGroupDataSet", "value": {"shortDescription": [{"value": "kg", "lang": "de"}], "type": "unit group data set", "refObjectId": "ad38d542-3fe9-439d-9b95-2f5f7752acaf", "uri": "../unitgroups/ad38d542-3fe9-439d-9b95-2f5f7752acaf.xml"}}, {"value": "0", "module": "A1-A3"}, {"value": "0", "module": "A4"}, {"value": "0", "module": "A5"}, {"module": "C1"}, {"value": "0", "module": "C2"}, {"value": "2.41", "module": "C3"}, {"value": "0", "module": "C4"}, {"value": "0", "module": "D"}]}, "resolvedFlowVersion": "38.00.000", "flowProperties": [], "typeOfFlow": "Other flow", "classification": {"classHierarchy": "Quantities / Environmental quantities / EPD EN 15804 / LCI indicators", "name": "GaBiCategories"}}, {"dataSetInternalID": 17, "referenceToFlowDataSet": {"shortDescription": [{"value": "Exportierte elektrische Energie (EEE)", "lang": "de"}, {"value": "Exported electrical energy (EEE)", "lang": "en"}], "type": "flow data set", "refObjectId": "4da0c987-2b76-40d6-9e9e-82a017aaaf29", "uri": "../flows/4da0c987-2b76-40d6-9e9e-82a017aaaf29.xml"}, "exchange direction": "OUTPUT", "other": {"anies": [{"name": "referenceToUnitGroupDataSet", "value": {"shortDescription": [{"value": "MJ", "lang": "de"}], "type": "unit group data set", "refObjectId": "93a60a57-a3c8-11da-a746-0800200c9a66", "uri": "../unitgroups/93a60a57-a3c8-11da-a746-0800200c9a66.xml"}}, {"value": "0", "module": "A1-A3"}, {"value": "0", "module": "A4"}, {"value": "0.413", "module": "A5"}, {"module": "C1"}, {"value": "0", "module": "C2"}, {"value": "0", "module": "C3"}, {"value": "0", "module": "C4"}, {"value": "-16.1", "module": "D"}]}, "resolvedFlowVersion": "38.00.000", "flowProperties": [], "typeOfFlow": "Other flow", "classification": {"classHierarchy": "Quantities / Environmental quantities / EPD EN 15804 / LCI indicators", "name": "GaBiCategories"}}, {"dataSetInternalID": 18, "referenceToFlowDataSet": {"shortDescription": [{"value": "Exportierte thermische Energie (EET)", "lang": "de"}, {"value": "Exported thermal energy (EET)", "lang": "en"}], "type": "flow data set", "refObjectId": "98daf38a-7a79-46d3-9a37-2b7bd0955810", "uri": "../flows/98daf38a-7a79-46d3-9a37-2b7bd0955810.xml"}, "exchange direction": "OUTPUT", "other": {"anies": [{"name": "referenceToUnitGroupDataSet", "value": {"shortDescription": [{"value": "MJ", "lang": "de"}], "type": "unit group data set", "refObjectId": "93a60a57-a3c8-11da-a746-0800200c9a66", "uri": "../unitgroups/93a60a57-a3c8-11da-a746-0800200c9a66.xml"}}, {"value": "0", "module": "A1-A3"}, {"value": "0", "module": "A4"}, {"value": "0.737", "module": "A5"}, {"module": "C1"}, {"value": "0", "module": "C2"}, {"value": "0", "module": "C3"}, {"value": "0", "module": "C4"}, {"value": "-28.6", "module": "D"}]}, "resolvedFlowVersion": "38.00.000", "flowProperties": [], "typeOfFlow": "Other flow", "classification": {"classHierarchy": "Quantities / Environmental quantities / EPD EN 15804 / LCI indicators", "name": "GaBiCategories"}}]}, "LCIAResults": {"LCIAResult": [{"referenceToLCIAMethodDataSet": {"shortDescription": [{"value": "Globales Erwärmungspotenzial total (GWP-total)", "lang": "de"}, {"value": "Global Warming Potential total (GWP-total)", "lang": "en"}], "type": "LCIA method data set", "refObjectId": "6a37f984-a4b3-458a-a20a-64418c145fa2", "uri": "../lciamethods/6a37f984-a4b3-458a-a20a-64418c145fa2.xml"}, "other": {"anies": [{"name": "referenceToUnitGroupDataSet", "value": {"shortDescription": [{"value": "kg CO_(2)-Äq.", "lang": "de"}], "type": "unit group data set", "refObjectId": "1ebf3012-d0db-4de2-aefd-ef30cedb0be1", "uri": "../unitgroups/1ebf3012-d0db-4de2-aefd-ef30cedb0be1.xml"}}, {"value": "2.18095238095238", "module": "A1-A3"}, {"value": "0.111428571428571", "module": "A4"}, {"value": "0.332619047619048", "module": "A5"}, {"module": "C1"}, {"value": "0.00916", "module": "C2"}, {"value": "7.54", "module": "C3"}, {"value": "0", "module": "C4"}, {"value": "-4.15", "module": "D"}]}}, {"referenceToLCIAMethodDataSet": {"shortDescription": [{"value": "Globales Erwärmungspotenzial fossil (GWP-fossil)", "lang": "de"}, {"value": "Global Warming Potential fossil fuels (GWP-fossil)", "lang": "en"}], "type": "LCIA method data set", "refObjectId": "5f635281-343e-44fb-83df-1971b155e6b6", "uri": "../lciamethods/5f635281-343e-44fb-83df-1971b155e6b6.xml"}, "other": {"anies": [{"name": "referenceToUnitGroupDataSet", "value": {"shortDescription": [{"value": "kg CO_(2)-Äq.", "lang": "de"}], "type": "unit group data set", "refObjectId": "1ebf3012-d0db-4de2-aefd-ef30cedb0be1", "uri": "../unitgroups/1ebf3012-d0db-4de2-aefd-ef30cedb0be1.xml"}}, {"value": "2.41904761904762", "module": "A1-A3"}, {"value": "0.111428571428571", "module": "A4"}, {"value": "0.29352380952381", "module": "A5"}, {"module": "C1"}, {"value": "0.00912", "module": "C2"}, {"value": "7.54", "module": "C3"}, {"value": "0", "module": "C4"}, {"value": "-4.3", "module": "D"}]}}, {"referenceToLCIAMethodDataSet": {"shortDescription": [{"value": "Globales Erwärmungspotenzial biogen (GWP-biogenic)", "lang": "de"}, {"value": "Global Warming Potential biogenic (GWP-biogenic)", "lang": "en"}], "type": "LCIA method data set", "refObjectId": "2356e1ab-0185-4db5-86e5-16de51c7485c", "uri": "../lciamethods/2356e1ab-0185-4db5-86e5-16de51c7485c.xml"}, "other": {"anies": [{"name": "referenceToUnitGroupDataSet", "value": {"shortDescription": [{"value": "kg CO_(2)-Äq.", "lang": "de"}], "type": "unit group data set", "refObjectId": "1ebf3012-d0db-4de2-aefd-ef30cedb0be1", "uri": "../unitgroups/1ebf3012-d0db-4de2-aefd-ef30cedb0be1.xml"}}, {"value": "-0.244761904761905", "module": "A1-A3"}, {"value": "-0.000153333333333333", "module": "A4"}, {"value": "0.0384542380952381", "module": "A5"}, {"module": "C1"}, {"value": "-1.26E-05", "module": "C2"}, {"value": "0.000242", "module": "C3"}, {"value": "0", "module": "C4"}, {"value": "0.146", "module": "D"}]}}, {"referenceToLCIAMethodDataSet": {"shortDescription": [{"value": "Globales Erwärmungspotenzial luluc (GWP-luluc)", "lang": "de"}, {"value": "Global Warming Potential luluc (GWP-luluc)", "lang": "en"}], "type": "LCIA method data set", "refObjectId": "4331bbdb-978a-490d-8707-eeb047f01a55", "uri": "../lciamethods/4331bbdb-978a-490d-8707-eeb047f01a55.xml"}, "other": {"anies": [{"name": "referenceToUnitGroupDataSet", "value": {"shortDescription": [{"value": "kg CO_(2)-Äq.", "lang": "de"}], "type": "unit group data set", "refObjectId": "1ebf3012-d0db-4de2-aefd-ef30cedb0be1", "uri": "../unitgroups/1ebf3012-d0db-4de2-aefd-ef30cedb0be1.xml"}}, {"value": "0.00128571428571429", "module": "A1-A3"}, {"value": "0.000617142857142857", "module": "A4"}, {"value": "0.000101642857142857", "module": "A5"}, {"module": "C1"}, {"value": "5.07E-05", "module": "C2"}, {"value": "7.96E-06", "module": "C3"}, {"value": "0", "module": "C4"}, {"value": "-0.000922", "module": "D"}]}}, {"referenceToLCIAMethodDataSet": {"shortDescription": [{"value": "Abbau Potential der stratosphärischen Ozonschicht (ODP)", "lang": "de"}, {"value": "Depletion potential of the stratospheric ozone layer (ODP)", "lang": "en"}], "type": "LCIA method data set", "refObjectId": "b5c629d6-def3-11e6-bf01-fe55135034f3", "uri": "../lciamethods/b5c629d6-def3-11e6-bf01-fe55135034f3.xml"}, "other": {"anies": [{"name": "referenceToUnitGroupDataSet", "value": {"shortDescription": [{"value": "kg CFC11-Äq.", "lang": "de"}], "type": "unit group data set", "refObjectId": "d9e957c9-7309-4474-bf3a-7777df6c4e5b", "uri": "../unitgroups/d9e957c9-7309-4474-bf3a-7777df6c4e5b.xml"}}, {"value": "1.37142857142857E-08", "module": "A1-A3"}, {"value": "6.63809523809524E-15", "module": "A4"}, {"value": "6.85894617619048E-10", "module": "A5"}, {"module": "C1"}, {"value": "5.45E-16", "module": "C2"}, {"value": "3.23E-13", "module": "C3"}, {"value": "0", "module": "C4"}, {"value": "-2.91E-09", "module": "D"}]}}, {"referenceToLCIAMethodDataSet": {"shortDescription": [{"value": "Versauerungspotenzial von Boden und Wasser (AP)", "lang": "de"}, {"value": "Acidification potential of land and water (AP)", "lang": "en"}], "type": "LCIA method data set", "refObjectId": "b5c611c6-def3-11e6-bf01-fe55135034f3", "uri": "../lciamethods/b5c611c6-def3-11e6-bf01-fe55135034f3.xml"}, "other": {"anies": [{"name": "referenceToUnitGroupDataSet", "value": {"shortDescription": [{"value": "mol H^(+)-Äq.", "lang": "de"}], "type": "unit group data set", "refObjectId": "42e089ac-92bf-4bf2-8ca1-5fc40d18f2ed", "uri": "../unitgroups/42e089ac-92bf-4bf2-8ca1-5fc40d18f2ed.xml"}}, {"value": "0.00665714285714286", "module": "A1-A3"}, {"value": "0.000107619047619048", "module": "A4"}, {"value": "0.000377738095238095", "module": "A5"}, {"module": "C1"}, {"value": "8.86E-06", "module": "C2"}, {"value": "0.000749", "module": "C3"}, {"value": "0", "module": "C4"}, {"value": "-0.00451", "module": "D"}]}}, {"referenceToLCIAMethodDataSet": {"shortDescription": [{"value": "Eutrophierungspotenzial Süßwasser (EP-freshwater)", "lang": "de"}, {"value": "Eutrophication potential aquatic freshwater (EP-freshwater)", "lang": "en"}], "type": "LCIA method data set", "refObjectId": "b53ec18f-7377-4ad3-86eb-cc3f4f276b2b", "uri": "../lciamethods/b53ec18f-7377-4ad3-86eb-cc3f4f276b2b.xml"}, "other": {"anies": [{"name": "referenceToUnitGroupDataSet", "value": {"shortDescription": [{"value": "kg P-Äq.", "lang": "de"}], "type": "unit group data set", "refObjectId": "0429039d-a61d-4590-ba67-aa4a20a810a1", "uri": "../unitgroups/0429039d-a61d-4590-ba67-aa4a20a810a1.xml"}}, {"value": "4.69523809523809E-05", "module": "A1-A3"}, {"value": "3.3047619047619E-07", "module": "A4"}, {"value": "2.40304285714286E-06", "module": "A5"}, {"module": "C1"}, {"value": "2.72E-08", "module": "C2"}, {"value": "7.53E-08", "module": "C3"}, {"value": "0", "module": "C4"}, {"value": "-1.7E-05", "module": "D"}]}}, {"referenceToLCIAMethodDataSet": {"shortDescription": [{"value": "Eutrophierungspotenzial Salzwasser (EP-marine)", "lang": "de"}, {"value": "Eutrophication potential aquatic marine (EP-marine)", "lang": "en"}], "type": "LCIA method data set", "refObjectId": "b5c619fa-def3-11e6-bf01-fe55135034f3", "uri": "../lciamethods/b5c619fa-def3-11e6-bf01-fe55135034f3.xml"}, "other": {"anies": [{"name": "referenceToUnitGroupDataSet", "value": {"shortDescription": [{"value": "kg N-Äq.", "lang": "de"}], "type": "unit group data set", "refObjectId": "d05bb823-ecdf-4686-8c40-bf1d9257859f", "uri": "../unitgroups/d05bb823-ecdf-4686-8c40-bf1d9257859f.xml"}}, {"value": "0.00154285714285714", "module": "A1-A3"}, {"value": "3.41904761904762E-05", "module": "A4"}, {"value": "9.02523809523809E-05", "module": "A5"}, {"module": "C1"}, {"value": "2.81E-06", "module": "C2"}, {"value": "0.000156", "module": "C3"}, {"value": "0", "module": "C4"}, {"value": "-0.00156", "module": "D"}]}}, {"referenceToLCIAMethodDataSet": {"shortDescription": [{"value": "Eutrophierungspotenzial Land (EP-terrestrial)", "lang": "de"}, {"value": "Eutrophication potential terrestrial (EP-terrestrial)", "lang": "en"}], "type": "LCIA method data set", "refObjectId": "b5c614d2-def3-11e6-bf01-fe55135034f3", "uri": "../lciamethods/b5c614d2-def3-11e6-bf01-fe55135034f3.xml"}, "other": {"anies": [{"name": "referenceToUnitGroupDataSet", "value": {"shortDescription": [{"value": "mol N-Äq.", "lang": "de"}], "type": "unit group data set", "refObjectId": "71b4d617-0ec9-4d3f-b65e-e438940c2401", "uri": "../unitgroups/71b4d617-0ec9-4d3f-b65e-e438940c2401.xml"}}, {"value": "0.0165714285714286", "module": "A1-A3"}, {"value": "0.000408571428571429", "module": "A4"}, {"value": "0.001018", "module": "A5"}, {"module": "C1"}, {"value": "3.36E-05", "module": "C2"}, {"value": "0.00351", "module": "C3"}, {"value": "0", "module": "C4"}, {"value": "-0.0166", "module": "D"}]}}, {"referenceToLCIAMethodDataSet": {"shortDescription": [{"value": "Bildungspotential für troposphärisches Ozon (POCP)", "lang": "de"}, {"value": "Formation potential of tropospheric ozone photochemical oxidants (POCP)", "lang": "en"}], "type": "LCIA method data set", "refObjectId": "b5c610fe-def3-11e6-bf01-fe55135034f3", "uri": "../lciamethods/b5c610fe-def3-11e6-bf01-fe55135034f3.xml"}, "other": {"anies": [{"name": "referenceToUnitGroupDataSet", "value": {"shortDescription": [{"value": "kg NMVOC-Äq.", "lang": "de"}], "type": "unit group data set", "refObjectId": "d27c25f8-fbc1-44c6-b47b-4adbae4199c6", "uri": "../unitgroups/d27c25f8-fbc1-44c6-b47b-4adbae4199c6.xml"}}, {"value": "0.00565714285714286", "module": "A1-A3"}, {"value": "9.43809523809524E-05", "module": "A4"}, {"value": "0.00031817619047619", "module": "A5"}, {"module": "C1"}, {"value": "7.75E-06", "module": "C2"}, {"value": "0.000465", "module": "C3"}, {"value": "0", "module": "C4"}, {"value": "-0.00413", "module": "D"}]}}, {"referenceToLCIAMethodDataSet": {"shortDescription": [{"value": "Potenzial für den abiotischen Abbau nicht fossiler Ressourcen (ADPE)", "lang": "de"}, {"value": "Abiotic depletion potential for non fossil resources (ADPE)", "lang": "en"}], "type": "LCIA method data set", "refObjectId": "b2ad6494-c78d-11e6-9d9d-cec0c932ce01", "uri": "../lciamethods/b2ad6494-c78d-11e6-9d9d-cec0c932ce01.xml"}, "other": {"anies": [{"name": "referenceToUnitGroupDataSet", "value": {"shortDescription": [{"value": "kg Sb-Äq.", "lang": "de"}], "type": "unit group data set", "refObjectId": "54ccd2d9-a32a-4fc2-923d-f2c8c93e89d4", "uri": "../unitgroups/54ccd2d9-a32a-4fc2-923d-f2c8c93e89d4.xml"}}, {"value": "2.87619047619048E-06", "module": "A1-A3"}, {"value": "9.25714285714286E-09", "module": "A4"}, {"value": "1.48142380952381E-07", "module": "A5"}, {"module": "C1"}, {"value": "7.6E-10", "module": "C2"}, {"value": "7.82E-09", "module": "C3"}, {"value": "0", "module": "C4"}, {"value": "-1.32E-06", "module": "D"}]}}, {"referenceToLCIAMethodDataSet": {"shortDescription": [{"value": "Potenzial für den abiotischen Abbau fossiler Brennstoffe (ADPF)", "lang": "de"}, {"value": "Abiotic depletion potential for fossil resources (ADPF)", "lang": "en"}], "type": "LCIA method data set", "refObjectId": "b2ad6110-c78d-11e6-9d9d-cec0c932ce01", "uri": "../lciamethods/b2ad6110-c78d-11e6-9d9d-cec0c932ce01.xml"}, "other": {"anies": [{"name": "referenceToUnitGroupDataSet", "value": {"shortDescription": [{"value": "MJ", "lang": "de"}], "type": "unit group data set", "refObjectId": "93a60a57-a3c8-11da-a746-0800200c9a66", "uri": "../unitgroups/93a60a57-a3c8-11da-a746-0800200c9a66.xml"}}, {"value": "71.6190476190476", "module": "A1-A3"}, {"value": "1.47619047619048", "module": "A4"}, {"value": "3.7937619047619", "module": "A5"}, {"module": "C1"}, {"value": "0.122", "module": "C2"}, {"value": "0.879", "module": "C3"}, {"value": "0", "module": "C4"}, {"value": "-61.1", "module": "D"}]}}, {"referenceToLCIAMethodDataSet": {"shortDescription": [{"value": "Wassernutzung (WDP)", "lang": "de"}, {"value": "Water use (WDP)", "lang": "en"}], "type": "LCIA method data set", "refObjectId": "b2ad66ce-c78d-11e6-9d9d-cec0c932ce01", "uri": "../lciamethods/b2ad66ce-c78d-11e6-9d9d-cec0c932ce01.xml"}, "other": {"anies": [{"name": "referenceToUnitGroupDataSet", "value": {"shortDescription": [{"value": "m^(3) Welt-Äq. entzogen", "lang": "de"}], "type": "unit group data set", "refObjectId": "6ae2df01-888e-46c8-b17d-49fa3869b476", "uri": "../unitgroups/6ae2df01-888e-46c8-b17d-49fa3869b476.xml"}}, {"value": "1.59047619047619", "module": "A1-A3"}, {"value": "0.00099047619047619", "module": "A4"}, {"value": "0.100373333333333", "module": "A5"}, {"module": "C1"}, {"value": "8.16E-05", "module": "C2"}, {"value": "0.696", "module": "C3"}, {"value": "0", "module": "C4"}, {"value": "-0.0759", "module": "D"}]}}, {"referenceToLCIAMethodDataSet": {"shortDescription": [{"value": "Auftreten von Krankheiten aufgrund von Feinstaubemissionen (PM)", "lang": "de"}, {"value": "Incidence of disease due to PM emissions (PM)", "lang": "en"}], "type": "LCIA method data set", "refObjectId": "b5c602c6-def3-11e6-bf01-fe55135034f3", "uri": "../lciamethods/b5c602c6-def3-11e6-bf01-fe55135034f3.xml"}, "other": {"anies": [{"name": "referenceToUnitGroupDataSet", "value": {"shortDescription": [{"value": "Krankheitsfälle", "lang": "de"}], "type": "unit group data set", "refObjectId": "3883559b-648f-4afc-8ba2-0bd24f3affa3", "uri": "../unitgroups/3883559b-648f-4afc-8ba2-0bd24f3affa3.xml"}}, {"value": "6.34285714285714E-08", "module": "A1-A3"}, {"value": "6.41904761904762E-10", "module": "A4"}, {"value": "2.36190476190476E-10", "module": "A5"}, {"module": "C1"}, {"value": "5.01904761904762E-11", "module": "C2"}, {"value": "4.16190476190476E-09", "module": "C3"}, {"value": "0", "module": "C4"}, {"value": "-3.5047619047619E-08", "module": "D"}]}}, {"referenceToLCIAMethodDataSet": {"shortDescription": [{"value": "Wirkung durch Exposition des Menschen mit U235 (IR)", "lang": "de"}, {"value": "Human exposure efficiency relative to U235 (IR)", "lang": "en"}], "type": "LCIA method data set", "refObjectId": "b5c632be-def3-11e6-bf01-fe55135034f3", "uri": "../lciamethods/b5c632be-def3-11e6-bf01-fe55135034f3.xml"}, "other": {"anies": [{"name": "referenceToUnitGroupDataSet", "value": {"shortDescription": [{"value": "kBq U235-Äq.", "lang": "de"}], "type": "unit group data set", "refObjectId": "456b05bf-1415-44a9-9993-02452f554c09", "uri": "../unitgroups/456b05bf-1415-44a9-9993-02452f554c09.xml"}}, {"value": "0.227619047619048", "module": "A1-A3"}, {"value": "0.000267619047619048", "module": "A4"}, {"value": "0.00111428571428571", "module": "A5"}, {"module": "C1"}, {"value": "2.0952380952381E-05", "module": "C2"}, {"value": "0.00831428571428571", "module": "C3"}, {"value": "0", "module": "C4"}, {"value": "-0.247619047619048", "module": "D"}]}}, {"referenceToLCIAMethodDataSet": {"shortDescription": [{"value": "Toxizitätsvergleichseinheit für Ökosysteme (ETP-fw)", "lang": "de"}, {"value": "Comparative toxic unit for ecosystems (ETP-fw)", "lang": "en"}], "type": "LCIA method data set", "refObjectId": "ee1082d1-b0f7-43ca-a1f0-21e2a4a74511", "uri": "../lciamethods/ee1082d1-b0f7-43ca-a1f0-21e2a4a74511.xml"}, "other": {"anies": [{"name": "referenceToUnitGroupDataSet", "value": {"shortDescription": [{"value": "CTUe", "lang": "de"}], "type": "unit group data set", "refObjectId": "aa959ded-f1eb-4efb-9c5c-2d60be36b3e6", "uri": "../unitgroups/aa959ded-f1eb-4efb-9c5c-2d60be36b3e6.xml"}}, {"value": "40.4761904761905", "module": "A1-A3"}, {"value": "1.02857142857143", "module": "A4"}, {"value": "0.0565714285714286", "module": "A5"}, {"module": "C1"}, {"value": "0.0803809523809524", "module": "C2"}, {"value": "0.387619047619048", "module": "C3"}, {"value": "0", "module": "C4"}, {"value": "-11.6190476190476", "module": "D"}]}}, {"referenceToLCIAMethodDataSet": {"shortDescription": [{"value": "Toxizitätsvergleichseinheit für Menschen (krebserregend) (HTP-c)", "lang": "de"}, {"value": "Comparative toxic unit for humans (carcinogenic) (HTP-c)", "lang": "en"}], "type": "LCIA method data set", "refObjectId": "2299222a-bbd8-474f-9d4f-4dd1f18aea7c", "uri": "../lciamethods/2299222a-bbd8-474f-9d4f-4dd1f18aea7c.xml"}, "other": {"anies": [{"name": "referenceToUnitGroupDataSet", "value": {"shortDescription": [{"value": "CTUh", "lang": "de"}], "type": "unit group data set", "refObjectId": "d4c9523e-2d7e-49fd-8469-998f547d3a70", "uri": "../unitgroups/d4c9523e-2d7e-49fd-8469-998f547d3a70.xml"}}, {"value": "1.17142857142857E-09", "module": "A1-A3"}, {"value": "2.06666666666667E-11", "module": "A4"}, {"value": "2.81904761904762E-12", "module": "A5"}, {"module": "C1"}, {"value": "1.61904761904762E-12", "module": "C2"}, {"value": "4.57142857142857E-11", "module": "C3"}, {"value": "0", "module": "C4"}, {"value": "-7.77142857142857E-10", "module": "D"}]}}, {"referenceToLCIAMethodDataSet": {"shortDescription": [{"value": "Toxizitätsvergleichseinheit für Menschen (nicht krebserregend) (HTP-nc)", "lang": "de"}, {"value": "Comparative toxic unit for humans (noncarcinogenic) (HTP-nc)", "lang": "en"}], "type": "LCIA method data set", "refObjectId": "3af763a5-b7a1-48c9-9cee-1f223481fcef", "uri": "../lciamethods/3af763a5-b7a1-48c9-9cee-1f223481fcef.xml"}, "other": {"anies": [{"name": "referenceToUnitGroupDataSet", "value": {"shortDescription": [{"value": "CTUh", "lang": "de"}], "type": "unit group data set", "refObjectId": "d4c9523e-2d7e-49fd-8469-998f547d3a70", "uri": "../unitgroups/d4c9523e-2d7e-49fd-8469-998f547d3a70.xml"}}, {"value": "5.51428571428571E-08", "module": "A1-A3"}, {"value": "1.07619047619048E-09", "module": "A4"}, {"value": "1.05714285714286E-10", "module": "A5"}, {"module": "C1"}, {"value": "8.4E-11", "module": "C2"}, {"value": "1.42857142857143E-09", "module": "C3"}, {"value": "0", "module": "C4"}, {"value": "-2.62857142857143E-08", "module": "D"}]}}, {"referenceToLCIAMethodDataSet": {"shortDescription": [{"value": "Bodenqualitätsindex (SQP)", "lang": "de"}, {"value": "Soil quality index (SQP)", "lang": "en"}], "type": "LCIA method data set", "refObjectId": "b2ad6890-c78d-11e6-9d9d-cec0c932ce01", "uri": "../lciamethods/b2ad6890-c78d-11e6-9d9d-cec0c932ce01.xml"}, "other": {"anies": [{"name": "referenceToUnitGroupDataSet", "value": {"shortDescription": [{"value": "SQP", "lang": "de"}], "type": "unit group data set", "refObjectId": "f130951c-e67f-4f7f-8dd4-665de3974e18", "uri": "../unitgroups/f130951c-e67f-4f7f-8dd4-665de3974e18.xml"}}, {"value": "18.2857142857143", "module": "A1-A3"}, {"value": "0.509523809523809", "module": "A4"}, {"value": "0.0622857142857143", "module": "A5"}, {"module": "C1"}, {"value": "0.0398095238095238", "module": "C2"}, {"value": "0.253333333333333", "module": "C3"}, {"value": "0", "module": "C4"}, {"value": "-24.5714285714286", "module": "D"}]}}]}, "otherAttributes": {"{http://www.indata.network/EPD/2019}epd-version": "1.2"}, "version": "1.1", "locations": "../ILCDLocations.xml"}