{"processInformation": {"dataSetInformation": {"UUID": "7312906e-da2d-4e38-9676-451caf72b1b7", "name": {"baseName": [{"value": "GRL 100 / GRP 300", "lang": "en"}, {"value": "GRL 100 / GRP 300", "lang": "de"}], "functionalUnitFlowProperties": [{"lang": "en"}]}, "classificationInformation": {"classification": [{"class": [{"value": "Komponenten von Fenstern und Vorhangfassaden", "level": 0, "classId": "7"}, {"value": "Antriebssysteme", "level": 1, "classId": "7.7"}, {"value": "mechanisch", "level": 2, "classId": "7.7.01"}], "name": "OEKOBAU.DAT"}, {"class": [{"value": "02 Building products", "level": 0}, {"value": "Doors, windows, shutters, and related products", "level": 1}, {"value": "Building Hardware products", "level": 2}], "name": "IBUCategories"}]}, "generalComment": [{"value": "The GRL 100 and GRP 300 series concealed door closers are dependable and versatile for almost any application. Their compact bodies enable them to be used in applications where larger closers would be prohibitive. They can be installed in a number of different configurations, including in standard, narrow or wide door frames, as well as with left-hand or right-hand single- or double-action mounting. The closers are designed for all types of doors and allow the necessary spring adjustments for both barrier-free and non-barrier free openings. A comprehensive selection of accessories ensures that they can be used successfully with a wide variety of door constructions and floor coverings. Product benefits include:\nFor the installer: Suitable for installation with left-hand or right-hand single and double action doors.\n\nFor the architect: Concealed installation for maximum visual elegance. A wide range of applications allow architects a reliable and durable solution without compromising the aesthetics of an opening.\nFor the user: A temperature-independent closing cycle and highly efficient mechanism gives maximum user convenience.", "lang": "en"}, {"value": "Die verdeckten Türschließer der Serien GRL 100 und GRP 300 sind zuverlässig und vielseitig für fast jede Anwendung geeignet. Dank ihrer kompakten Bauweise können sie auch dort eingesetzt werden, wo größere Schließer unpraktisch wären. Sie können in verschiedenen Konfigurationen eingebaut werden, z.B. in Standard-, schmale oder breite Türrahmen, sowie mit linker oder rechter Montage mit einfacher oder doppelter Betätigung. Die Schließer sind für alle Arten von Türen geeignet und ermöglichen die notwendigen Federeinstellungen für barrierefreie und nicht barrierefreie Öffnungen. Eine umfangreiche Auswahl an Zubehör sorgt dafür, dass sie mit einer Vielzahl von Türkonstruktionen und Bodenbelägen erfolgreich eingesetzt werden können. Die Produktvorteile umfassen: Für den Installateur: Geeignet für den Einbau in links oder rechts angeschlagene ein- und zweiflügelige Türen. Für den Architekten: Verdeckter Einbau für maximale optische Eleganz. Eine breite Palette von Anwendungen ermöglicht Architekten eine zuverlässige und dauerhafte Lösung, ohne die Ästhetik einer Öffnung zu beeinträchtigen. Für den Benutzer: Ein temperaturunabhängiger Schließzyklus und ein hocheffizienter Mechanismus sorgen für maximalen Benutzerkomfort.", "lang": "de"}]}, "quantitativeReference": {"referenceToReferenceFlow": [0]}, "time": {"referenceYear": 2020, "dataSetValidUntil": 2025, "other": {"anies": [{"name": "publicationDateOfEPD", "value": 1598227200000}]}}, "geography": {"locationOfOperationSupplyOrProduction": {"location": "SG"}}, "technology": {"technologyDescriptionAndIncludedProcesses": [{"value": "The GRL 100 and GRP 300 series concealed door closers are dependable and versatile for almost any application. Their compact bodies enable them to be used in applications where larger closers would be prohibitive. They can be installed in a number of different configurations, including in standard, narrow or wide door frames, as well as with left-hand or righthand single- or double-action mounting. The closers are designed for all types of doors and allow the necessary spring adjustments for both barrier-free and non-barrier free openings. A comprehensive selection of accessories ensures that they can be used successfully with a wide variety of door constructions and floor coverings. \nTechnical data: \nThe concealed door closers employ a cam and roller mechanism, and are capable of controlling interior or exterior doors weighing up to 120 kg. They have an adjustable closing force from EN 1 to EN 4 and a mechanical backcheck at approximately 70°. Dual valve adjustment provides a controlled closing speed from approximately 175° opening range, even in cold temperature conditions.\nThe plant in\nSingapore is certified to the quality management system ISO 9001, which\nensures consistent quality of the products. The Environmental Management System in the\nSingapore production is certified to ISO 14001 and the Energy Management\nto ISO 50001. \nDeclared unit: \nThe declared unit of this analysis is one concealed door closer.", "lang": "en"}, {"value": "Die verdeckten Türschließer der Serien GRL 100 und GRP 300 sind zuverlässig und vielseitig für nahezu jede Anwendung geeignet. Dank ihrer kompakten Bauweise können sie auch dort eingesetzt werden, wo größere Schließer unpraktisch wären. Sie können in verschiedenen Konfigurationen installiert werden, z. B. in Standard-, schmalen oder breiten Türrahmen sowie mit einfachem oder doppeltem Antrieb für die linke oder rechte Seite. Die Schließer sind für alle Türarten geeignet und ermöglichen die notwendigen Federeinstellungen für barrierefreie und nicht barrierefreie Öffnungen. Eine umfangreiche Auswahl an Zubehör sorgt dafür, dass sie mit einer Vielzahl von Türkonstruktionen und Bodenbelägen erfolgreich eingesetzt werden können. \nTechnische Daten: \nDie verdeckten Türschließer arbeiten mit einem Nocken- und Rollenmechanismus und sind in der Lage, Innen- oder Außentüren mit einem Gewicht von bis zu 120 kg zu bedienen. Sie haben eine einstellbare Schließkraft von EN 1 bis EN 4 und eine mechanische Rücklaufsperre bei ca. 70°. Die doppelte Ventileinstellung sorgt für eine kontrollierte Schließgeschwindigkeit ab einem Öffnungsbereich von ca. 175°, auch bei kalten Temperaturen. Das Werk in Singapur ist nach dem Qualitätsmanagementsystem ISO 9001 zertifiziert, das eine gleichbleibende Qualität der Produkte gewährleistet. Das Umweltmanagementsystem in der Produktion in Singapur ist nach ISO 14001 und das Energiemanagement nach ISO 50001 zertifiziert. \nDeklarierte Einheit: \nDie erklärte Einheit dieser Analyse ist ein verdeckter Türschließer.", "lang": "de"}], "technologicalApplicability": [{"value": "The GRL 100 and GRP 300 series offer aesthetically pleasing solutions for both interior and exterior applications. The closers can be used in a variety of applications, including as closers\nfor fire and smoke doors for the non-hold-open versions.", "lang": "en"}, {"value": "Die Serien GRL 100 und GRP 300 bieten ästhetisch ansprechende Lösungen für Innen- und Außenanwendungen. Die Schließer können in einer Vielzahl von Anwendungen eingesetzt werden, u.a. als Schließer für Feuer- und Rauchschutztüren bei den Versionen ohne Feststellanlage.", "lang": "de"}]}}, "modellingAndValidation": {"LCIMethodAndAllocation": {"typeOfDataSet": "EPD", "referenceToLCAMethodDetails": [{"shortDescription": [{"value": "Building Hardware products.pdf", "lang": "en"}], "type": "source data set", "refObjectId": "74179b0b-9435-4269-8069-9a99988834cb"}], "other": {"anies": [{"name": "subType", "value": "average dataset"}]}}, "dataSourcesTreatmentAndRepresentativeness": {"referenceToDataSource": [{"shortDescription": [{"value": "GaBi Database (all versions)", "lang": "en"}], "type": "source data set", "refObjectId": "28d74cc0-db8b-4d7e-bc44-5f6d56ce0c4a"}, {"shortDescription": [{"value": "GaBi database SP39 2019", "lang": "en"}], "type": "source data set", "refObjectId": "07d9b8a7-e0fc-408f-a95e-c90735f843ce"}], "useAdviceForDataSet": [{"value": "Scope: \nThe declaration and the background LCA represent GROOM's GRL 100 and GRP 300 Series Concealed Door Closers. Raw materials and components are provided by suppliers and shipped Singapore, where the closers are manufactured and assembled. The GRL 100 and GRP 300 differ in how they are mounted to the door (floor versus frame), but are otherwise identical products. \nSystem boundary: \nType of EPD:\ncradle to gate - with options.\n\n\nThe\nEnvironmental Product Declaration refers to the production stage (A1-A3), transport from the gate to\nconstruction site (A4), the end of life stage (C3) and indicates the recycling\npotential which is declared in the module \"benefits and loads beyond the\nproduct system boundary\" (D).\n\n\nIn line with\nthe PCR, A5 is declared to ensure the export of biogenic CO2 from\nrenewable packaging materials.\n\n\n\nModules A1 to\nA3 include the provision and processing of raw materials as well as the\nprocessing of input materials, the transport to manufacturer and production\nsite.  Module C3 includes the incineration of plastics for\nenergy recovery. Module D comprises the recycling of metals and gives\nthe recycling potentials as well as potential benefits from energy\nsubstitution.\n\nA5 is declared to ensure the export of biogenic CO2\nthat is incorporated in the used packaging materials (paper). Potential benefits\nfrom the incineration of packaging materials are also declared in module D. The incineration processes in the End-of-Life are based on European datasets. The recycling processes in the End-of-Life are based on European and Global datasets.", "lang": "en"}, {"value": "Gültigkeitsbereich: \nDie Deklaration und die Hintergrund-Ökobilanz beziehen sich auf GROOMs verdeckte Türschließer der Serien GRL 100 und GRP 300. Die Rohstoffe und Komponenten werden von Lieferanten geliefert und nach Singapur verschifft, wo die Schließer hergestellt und montiert werden. Der GRL 100 und der GRP 300 unterscheiden sich in der Art und Weise, wie sie an der Tür montiert werden (Boden oder Rahmen), sind aber ansonsten identische Produkte. \nSystemgrenze: \nArt der EPD: cradle to gate - mit Optionen. Die Umweltproduktdeklaration bezieht sich auf die Produktionsstufe (A1-A3), den Transport vom Werkstor bis zur Baustelle (A4), die End-of-Life-Stufe (C3) und gibt das Recyclingpotenzial an, das im Modul \"Nutzen und Lasten über die Produktsystemgrenze hinaus\" (D) deklariert wird. In Übereinstimmung mit der PCR wird A5 deklariert, um den Export von biogenem CO2 aus erneuerbaren Verpackungsmaterialien zu gewährleisten. Die Module A1 bis A3 umfassen die Bereitstellung und Verarbeitung von Rohstoffen sowie die Verarbeitung von Vormaterialien, den Transport zum Hersteller und zur Produktionsstätte.  Modul C3 umfasst die Verbrennung von Kunststoffen zur Energierückgewinnung. Modul D umfasst das Recycling von Metallen und gibt die Recyclingpotenziale sowie den potenziellen Nutzen aus der Energiesubstitution an. A5 wird angegeben, um den Export von biogenem CO2 sicherzustellen, das in den verwendeten Verpackungsmaterialien (Papier) enthalten ist. Potenzielle Vorteile aus der Verbrennung von Verpackungsmaterialien werden auch in Modul D angegeben. Die Verbrennungsprozesse im End-of-Life-Bereich basieren auf europäischen Datensätzen. Die Recyclingprozesse am Ende des Lebenszyklus basieren auf europäischen und globalen Daten.", "lang": "de"}], "other": {"anies": [{"name": "referenceToOriginalEPD", "value": {"shortDescription": {"value": "GRL 100 / GRP 300.pdf", "defaultValue": "GRL 100 / GRP 300.pdf", "lstrings": [{"lang": "en", "value": "GRL 100 / GRP 300.pdf"}]}, "type": "source data set", "uuid": {"uuid": "5caa2f9c-82f4-4e4f-856e-4772cbc1bb1d"}, "refObjectId": "5caa2f9c-82f4-4e4f-856e-4772cbc1bb1d", "resourceURLs": ["https://oekobaudat.de/OEKOBAU.DAT/resource/sources/5caa2f9c-82f4-4e4f-856e-4772cbc1bb1d/GRL_100_GRP_300_13070.pdf?version=00.01.000"]}}]}}, "validation": {"review": [{"referenceToNameOfReviewerAndInstitution": [{"shortDescription": [{"value": "Institut Bauen und Umwelt e. V.", "lang": "en"}], "type": "contact data set", "refObjectId": "d111dbec-b024-4be5-86c5-752d6eb2cf95", "uri": "../contacts/d111dbec-b024-4be5-86c5-752d6eb2cf95.xml"}], "type": "Accredited third party review"}]}, "complianceDeclarations": {"compliance": [{"referenceToComplianceSystem": {"shortDescription": [{"value": "DIN EN 15804", "lang": "en"}], "type": "source data set", "refObjectId": "b00f9ec0-7874-11e3-981f-0800200c9a66", "uri": "../sources/b00f9ec0-7874-11e3-981f-0800200c9a66.xml"}}, {"referenceToComplianceSystem": {"shortDescription": [{"value": "ISO 14025", "lang": "en"}], "type": "source data set", "refObjectId": "4f2eb655-6e44-4874-a95a-e28f5442cd4d", "uri": "../sources/4f2eb655-6e44-4874-a95a-e28f5442cd4d.xml"}}]}}, "administrativeInformation": {"commissionerAndGoal": {"referenceToCommissioner": [{"shortDescription": [{"value": "dormakaba International Holding GmbH", "lang": "en"}], "type": "contact data set", "refObjectId": "33313944-7b37-498a-b458-25a295c1017d", "uri": "../contacts/33313944-7b37-498a-b458-25a295c1017d.xml"}]}, "dataGenerator": {"referenceToPersonOrEntityGeneratingTheDataSet": [{"shortDescription": [{"value": "Sphera Solutions GmbH", "lang": "en"}], "type": "contact data set", "refObjectId": "623edf96-39d1-4e6f-9892-674c7228546b", "uri": "../contacts/623edf96-39d1-4e6f-9892-674c7228546b.xml"}]}, "dataEntryBy": {"timeStamp": 1598227200000, "referenceToDataSetFormat": [{"shortDescription": [{"value": "ILCD Format", "lang": "en"}], "type": "source data set", "refObjectId": "a97a0155-0234-4b87-b4ce-a45da52f2a40", "uri": "../sources/a97a0155-0234-4b87-b4ce-a45da52f2a40.xml"}, {"shortDescription": [{"value": "EPD-Datenformaterweiterungen v1.2", "lang": "de"}, {"value": "EPD Data Format Extensions v1.2", "lang": "en"}], "type": "source data set", "refObjectId": "a29449fd-aa2f-4de8-b5d7-4b06b43c6fde", "uri": "../sources/a29449fd-aa2f-4de8-b5d7-4b06b43c6fde.xml"}]}, "publicationAndOwnership": {"dataSetVersion": "00.01.000", "referenceToRegistrationAuthority": {"shortDescription": [{"value": "Institut Bauen und Umwelt e. V.", "lang": "en"}], "type": "contact data set", "refObjectId": "d111dbec-b024-4be5-86c5-752d6eb2cf95", "uri": "../contacts/d111dbec-b024-4be5-86c5-752d6eb2cf95.xml"}, "registrationNumber": "EPD-GRO-20200245-CBD1-EN", "referenceToOwnershipOfDataSet": {"shortDescription": [{"value": "dormakaba International Holding GmbH", "lang": "en"}], "type": "contact data set", "refObjectId": "33313944-7b37-498a-b458-25a295c1017d", "uri": "../contacts/33313944-7b37-498a-b458-25a295c1017d.xml"}, "copyright": true, "licenseType": "Free of charge for all users and uses", "accessRestrictions": [{"value": "None", "lang": "en"}], "other": {"anies": [{"name": "referenceToPublisher", "value": {"shortDescription": [{"value": "Institut Bauen und Umwelt e. V.", "lang": "en"}], "type": "contact data set", "refObjectId": "d111dbec-b024-4be5-86c5-752d6eb2cf95", "uri": "../contacts/d111dbec-b024-4be5-86c5-752d6eb2cf95.xml"}}]}}}, "exchanges": {"exchange": [{"dataSetInternalID": 0, "referenceToFlowDataSet": {"shortDescription": [{"value": "GRL 100 / GRP 300 ()", "lang": "en"}], "type": "flow data set", "refObjectId": "2ff909e4-028a-5007-e602-a81b080bd993", "uri": "../flows/2ff909e4-028a-5007-e602-a81b080bd993.xml"}, "meanAmount": 1.0, "referencesToDataSource": {}, "referenceFlow": true, "resolvedFlowVersion": "00.01.000", "resultingflowAmount": 1.0, "flowProperties": [{"name": [{"lang": "de", "value": "Anzahl"}, {"lang": "en", "value": "Number of pieces"}], "uuid": "01846770-4cfe-4a25-8ad9-919d8d378345", "referenceFlowProperty": true, "meanValue": 1.0, "referenceUnit": "pcs.", "unitGroupUUID": "934110e3-baf4-49e9-992c-3d8109a6aafb"}, {"name": [{"lang": "en", "value": "Weight"}], "uuid": "93a60a56-a3c8-11da-a746-0800200b9a66", "meanValue": 2.9}], "materialProperties": [{"name": "weight per piece", "value": "2.9", "unit": "kg"}], "typeOfFlow": "Product flow", "classification": {"classHierarchy": "Komponenten von Fenstern und Vorhangfassaden / Antriebssysteme / mechanisch", "name": "OEKOBAU.DAT"}}, {"dataSetInternalID": 1, "referenceToFlowDataSet": {"shortDescription": [{"value": "Renewable primary energy as energy carrier (PERE)", "lang": "en"}, {"value": "Erneuerbare Primärenergie als Energieträger (PERE)", "lang": "de"}], "type": "flow data set", "refObjectId": "20f32be5-0398-4288-9b6d-accddd195317", "uri": "../flows/20f32be5-0398-4288-9b6d-accddd195317.xml"}, "exchange direction": "INPUT", "other": {"anies": [{"name": "referenceToUnitGroupDataSet", "value": {"shortDescription": [{"value": "MJ", "lang": "en"}], "type": "unit group data set", "refObjectId": "93a60a57-a3c8-11da-a746-0800200c9a66", "uri": "../unitgroups/93a60a57-a3c8-11da-a746-0800200c9a66.xml"}}, {"value": "55.2", "module": "A1-A3"}, {"value": "0.0318", "module": "A4"}, {"value": "1.809", "module": "A5"}, {"value": "0.0259", "module": "C3"}, {"value": "-34.9", "module": "D"}]}, "resolvedFlowVersion": "38.00.000", "flowProperties": [], "typeOfFlow": "Other flow", "classification": {"classHierarchy": "Quantities", "name": "GaBiCategories"}}, {"dataSetInternalID": 2, "referenceToFlowDataSet": {"shortDescription": [{"value": "Renewable primary energy resources as material utilization (PERM)", "lang": "en"}, {"value": "Erneuerbare Primärenergie zur stofflichen Nutzung (PERM)", "lang": "de"}], "type": "flow data set", "refObjectId": "fb3ec0de-548d-4508-aea5-00b73bf6f702", "uri": "../flows/fb3ec0de-548d-4508-aea5-00b73bf6f702.xml"}, "exchange direction": "INPUT", "other": {"anies": [{"name": "referenceToUnitGroupDataSet", "value": {"shortDescription": [{"value": "MJ", "lang": "en"}], "type": "unit group data set", "refObjectId": "93a60a57-a3c8-11da-a746-0800200c9a66", "uri": "../unitgroups/93a60a57-a3c8-11da-a746-0800200c9a66.xml"}}, {"value": "1.8", "module": "A1-A3"}, {"value": "0", "module": "A4"}, {"value": "-1.8", "module": "A5"}, {"value": "0", "module": "C3"}, {"value": "0", "module": "D"}]}, "resolvedFlowVersion": "38.00.000", "flowProperties": [], "typeOfFlow": "Other flow", "classification": {"classHierarchy": "Quantities", "name": "GaBiCategories"}}, {"dataSetInternalID": 3, "referenceToFlowDataSet": {"shortDescription": [{"value": "Total use of renewable primary energy resources (PERT)", "lang": "en"}, {"value": "Total erneuerbare Primärenergie (PERT)", "lang": "de"}], "type": "flow data set", "refObjectId": "53f97275-fa8a-4cdd-9024-65936002acd0", "uri": "../flows/53f97275-fa8a-4cdd-9024-65936002acd0.xml"}, "exchange direction": "INPUT", "other": {"anies": [{"name": "referenceToUnitGroupDataSet", "value": {"shortDescription": [{"value": "MJ", "lang": "en"}], "type": "unit group data set", "refObjectId": "93a60a57-a3c8-11da-a746-0800200c9a66", "uri": "../unitgroups/93a60a57-a3c8-11da-a746-0800200c9a66.xml"}}, {"value": "57", "module": "A1-A3"}, {"value": "0.0318", "module": "A4"}, {"value": "0.00943", "module": "A5"}, {"value": "0.0259", "module": "C3"}, {"value": "-34.9", "module": "D"}]}, "resolvedFlowVersion": "38.00.000", "flowProperties": [], "typeOfFlow": "Other flow", "classification": {"classHierarchy": "Quantities / Environmental quantities / EPD EN 15804 / LCI indicators", "name": "GaBiCategories"}}, {"dataSetInternalID": 4, "referenceToFlowDataSet": {"shortDescription": [{"value": "Non renewable primary energy as energy carrier (PENRE)", "lang": "en"}, {"value": "Nicht-erneuerbare Primärenergie als Energieträger (PENRE)", "lang": "de"}], "type": "flow data set", "refObjectId": "ac857178-2b45-46ec-892a-a9a4332f0372", "uri": "../flows/ac857178-2b45-46ec-892a-a9a4332f0372.xml"}, "exchange direction": "INPUT", "other": {"anies": [{"name": "referenceToUnitGroupDataSet", "value": {"shortDescription": [{"value": "MJ", "lang": "en"}], "type": "unit group data set", "refObjectId": "93a60a57-a3c8-11da-a746-0800200c9a66", "uri": "../unitgroups/93a60a57-a3c8-11da-a746-0800200c9a66.xml"}}, {"value": "212.37", "module": "A1-A3"}, {"value": "0", "module": "A4"}, {"value": "0", "module": "A5"}, {"value": "1.741", "module": "C3"}, {"value": "0", "module": "D"}]}, "resolvedFlowVersion": "38.00.000", "flowProperties": [], "typeOfFlow": "Other flow", "classification": {"classHierarchy": "Quantities", "name": "GaBiCategories"}}, {"dataSetInternalID": 5, "referenceToFlowDataSet": {"shortDescription": [{"value": "Non renewable primary energy as material utilization (PENRM)", "lang": "en"}, {"value": "Nicht-erneuerbare Primärenergie zur stofflichen Nutzung (PENRM)", "lang": "de"}], "type": "flow data set", "refObjectId": "1421caa0-679d-4bf4-b282-0eb850ccae27", "uri": "../flows/1421caa0-679d-4bf4-b282-0eb850ccae27.xml"}, "exchange direction": "INPUT", "other": {"anies": [{"name": "referenceToUnitGroupDataSet", "value": {"shortDescription": [{"value": "MJ", "lang": "en"}], "type": "unit group data set", "refObjectId": "93a60a57-a3c8-11da-a746-0800200c9a66", "uri": "../unitgroups/93a60a57-a3c8-11da-a746-0800200c9a66.xml"}}, {"value": "1.63", "module": "A1-A3"}, {"value": "0", "module": "A4"}, {"value": "0", "module": "A5"}, {"value": "-1.63", "module": "C3"}, {"value": "0", "module": "D"}]}, "resolvedFlowVersion": "38.00.000", "flowProperties": [], "typeOfFlow": "Other flow", "classification": {"classHierarchy": "Quantities", "name": "GaBiCategories"}}, {"dataSetInternalID": 6, "referenceToFlowDataSet": {"shortDescription": [{"value": "Total use of non renewable primary energy resources (PENRT)", "lang": "en"}, {"value": "Total nicht erneuerbare Primärenergie (PENRT)", "lang": "de"}], "type": "flow data set", "refObjectId": "06159210-646b-4c8d-8583-da9b3b95a6c1", "uri": "../flows/06159210-646b-4c8d-8583-da9b3b95a6c1.xml"}, "exchange direction": "INPUT", "other": {"anies": [{"name": "referenceToUnitGroupDataSet", "value": {"shortDescription": [{"value": "MJ", "lang": "en"}], "type": "unit group data set", "refObjectId": "93a60a57-a3c8-11da-a746-0800200c9a66", "uri": "../unitgroups/93a60a57-a3c8-11da-a746-0800200c9a66.xml"}}, {"value": "214", "module": "A1-A3"}, {"value": "8.63", "module": "A4"}, {"value": "0.0552", "module": "A5"}, {"value": "0.111", "module": "C3"}, {"value": "-116", "module": "D"}]}, "resolvedFlowVersion": "38.00.000", "flowProperties": [], "typeOfFlow": "Other flow", "classification": {"classHierarchy": "Quantities / Environmental quantities / EPD EN 15804 / LCI indicators", "name": "GaBiCategories"}}, {"dataSetInternalID": 7, "referenceToFlowDataSet": {"shortDescription": [{"value": "Use of secondary material (SM)", "lang": "en"}, {"value": "Einsatz von Sekundärstoffen (SM)", "lang": "de"}], "type": "flow data set", "refObjectId": "c6a1f35f-2d09-4f54-8dfb-97e502e1ce92", "uri": "../flows/c6a1f35f-2d09-4f54-8dfb-97e502e1ce92.xml"}, "exchange direction": "INPUT", "other": {"anies": [{"name": "referenceToUnitGroupDataSet", "value": {"shortDescription": [{"value": "kg", "lang": "en"}], "type": "unit group data set", "refObjectId": "ad38d542-3fe9-439d-9b95-2f5f7752acaf", "uri": "../unitgroups/ad38d542-3fe9-439d-9b95-2f5f7752acaf.xml"}}, {"value": "1.11", "module": "A1-A3"}, {"value": "0", "module": "A4"}, {"value": "0", "module": "A5"}, {"value": "0", "module": "C3"}, {"value": "0", "module": "D"}]}, "resolvedFlowVersion": "38.00.000", "flowProperties": [], "typeOfFlow": "Other flow", "classification": {"classHierarchy": "Quantities / Environmental quantities / EPD EN 15804 / LCI indicators", "name": "GaBiCategories"}}, {"dataSetInternalID": 8, "referenceToFlowDataSet": {"shortDescription": [{"value": "Use of renewable secondary fuels (RSF)", "lang": "en"}, {"value": "Erneuerbare Sekundärbrennstoffe (RSF)", "lang": "de"}], "type": "flow data set", "refObjectId": "64333088-a55f-4aa2-9a31-c10b07816787", "uri": "../flows/64333088-a55f-4aa2-9a31-c10b07816787.xml"}, "exchange direction": "INPUT", "other": {"anies": [{"name": "referenceToUnitGroupDataSet", "value": {"shortDescription": [{"value": "MJ", "lang": "en"}], "type": "unit group data set", "refObjectId": "93a60a57-a3c8-11da-a746-0800200c9a66", "uri": "../unitgroups/93a60a57-a3c8-11da-a746-0800200c9a66.xml"}}, {"value": "0", "module": "A1-A3"}, {"value": "0", "module": "A4"}, {"value": "0", "module": "A5"}, {"value": "0", "module": "C3"}, {"value": "0", "module": "D"}]}, "resolvedFlowVersion": "38.00.000", "flowProperties": [], "typeOfFlow": "Other flow", "classification": {"classHierarchy": "Quantities / Environmental quantities / EPD EN 15804 / LCI indicators", "name": "GaBiCategories"}}, {"dataSetInternalID": 9, "referenceToFlowDataSet": {"shortDescription": [{"value": "Use of non renewable secondary fuels (NRSF)", "lang": "en"}, {"value": "Nicht erneuerbare Sekundärbrennstoffe (NRSF)", "lang": "de"}], "type": "flow data set", "refObjectId": "89def144-d39a-4287-b86f-efde453ddcb2", "uri": "../flows/89def144-d39a-4287-b86f-efde453ddcb2.xml"}, "exchange direction": "INPUT", "other": {"anies": [{"name": "referenceToUnitGroupDataSet", "value": {"shortDescription": [{"value": "MJ", "lang": "en"}], "type": "unit group data set", "refObjectId": "93a60a57-a3c8-11da-a746-0800200c9a66", "uri": "../unitgroups/93a60a57-a3c8-11da-a746-0800200c9a66.xml"}}, {"value": "0", "module": "A1-A3"}, {"value": "0", "module": "A4"}, {"value": "0", "module": "A5"}, {"value": "0", "module": "C3"}, {"value": "0", "module": "D"}]}, "resolvedFlowVersion": "38.00.000", "flowProperties": [], "typeOfFlow": "Other flow", "classification": {"classHierarchy": "Quantities / Environmental quantities / EPD EN 15804 / LCI indicators", "name": "GaBiCategories"}}, {"dataSetInternalID": 10, "referenceToFlowDataSet": {"shortDescription": [{"value": "Use of net fresh water (FW)", "lang": "en"}, {"value": "Einsatz von Süßwasserressourcen (FW)", "lang": "de"}], "type": "flow data set", "refObjectId": "3cf952c8-f3a4-461d-8c96-96456ca62246", "uri": "../flows/3cf952c8-f3a4-461d-8c96-96456ca62246.xml"}, "exchange direction": "INPUT", "other": {"anies": [{"name": "referenceToUnitGroupDataSet", "value": {"shortDescription": [{"value": "m^3", "lang": "en"}], "type": "unit group data set", "refObjectId": "cd950537-0a98-4044-9ba7-9f9a68d0a504", "uri": "../unitgroups/cd950537-0a98-4044-9ba7-9f9a68d0a504.xml"}}, {"value": "0.142", "module": "A1-A3"}, {"value": "0.000147", "module": "A4"}, {"value": "0.000497", "module": "A5"}, {"value": "0.00068", "module": "C3"}, {"value": "-0.102", "module": "D"}]}, "resolvedFlowVersion": "38.00.000", "flowProperties": [], "typeOfFlow": "Other flow", "classification": {"classHierarchy": "Quantities / Environmental quantities / EPD EN 15804 / LCI indicators", "name": "GaBiCategories"}}, {"dataSetInternalID": 11, "referenceToFlowDataSet": {"shortDescription": [{"value": "Hazardous waste disposed (HWD)", "lang": "en"}, {"value": "Gefährlicher Abfall zur Deponie (HWD)", "lang": "de"}], "type": "flow data set", "refObjectId": "430f9e0f-59b2-46a0-8e0d-55e0e84948fc", "uri": "../flows/430f9e0f-59b2-46a0-8e0d-55e0e84948fc.xml"}, "exchange direction": "OUTPUT", "other": {"anies": [{"name": "referenceToUnitGroupDataSet", "value": {"shortDescription": [{"value": "kg", "lang": "en"}], "type": "unit group data set", "refObjectId": "ad38d542-3fe9-439d-9b95-2f5f7752acaf", "uri": "../unitgroups/ad38d542-3fe9-439d-9b95-2f5f7752acaf.xml"}}, {"value": "6.62E-06", "module": "A1-A3"}, {"value": "1.12E-09", "module": "A4"}, {"value": "1.07E-10", "module": "A5"}, {"value": "9.35E-10", "module": "C3"}, {"value": "-3E-07", "module": "D"}]}, "resolvedFlowVersion": "38.00.000", "flowProperties": [], "typeOfFlow": "Other flow", "classification": {"classHierarchy": "Quantities / Environmental quantities / EPD EN 15804 / LCI indicators", "name": "GaBiCategories"}}, {"dataSetInternalID": 12, "referenceToFlowDataSet": {"shortDescription": [{"value": "Non hazardous waste disposed (NHWD)", "lang": "en"}, {"value": "Entsorgter nicht gefährlicher Abfall (NHWD)", "lang": "de"}], "type": "flow data set", "refObjectId": "b29ef66b-e286-4afa-949f-62f1a7b4d7fa", "uri": "../flows/b29ef66b-e286-4afa-949f-62f1a7b4d7fa.xml"}, "exchange direction": "OUTPUT", "other": {"anies": [{"name": "referenceToUnitGroupDataSet", "value": {"shortDescription": [{"value": "kg", "lang": "en"}], "type": "unit group data set", "refObjectId": "ad38d542-3fe9-439d-9b95-2f5f7752acaf", "uri": "../unitgroups/ad38d542-3fe9-439d-9b95-2f5f7752acaf.xml"}}, {"value": "2.68", "module": "A1-A3"}, {"value": "6.57E-05", "module": "A4"}, {"value": "0.00534", "module": "A5"}, {"value": "0.0172", "module": "C3"}, {"value": "-1.8", "module": "D"}]}, "resolvedFlowVersion": "38.00.000", "flowProperties": [], "typeOfFlow": "Other flow", "classification": {"classHierarchy": "Quantities / Environmental quantities / EPD EN 15804 / LCI indicators", "name": "GaBiCategories"}}, {"dataSetInternalID": 13, "referenceToFlowDataSet": {"shortDescription": [{"value": "Radioactive waste disposed (RWD)", "lang": "en"}, {"value": "Entsorgter radioaktiver Abfall (RWD)", "lang": "de"}], "type": "flow data set", "refObjectId": "3449546e-52ad-4b39-b809-9fb77cea8ff6", "uri": "../flows/3449546e-52ad-4b39-b809-9fb77cea8ff6.xml"}, "exchange direction": "OUTPUT", "other": {"anies": [{"name": "referenceToUnitGroupDataSet", "value": {"shortDescription": [{"value": "kg", "lang": "en"}], "type": "unit group data set", "refObjectId": "ad38d542-3fe9-439d-9b95-2f5f7752acaf", "uri": "../unitgroups/ad38d542-3fe9-439d-9b95-2f5f7752acaf.xml"}}, {"value": "0.00775", "module": "A1-A3"}, {"value": "3.02E-06", "module": "A4"}, {"value": "3.2E-06", "module": "A5"}, {"value": "4.6E-06", "module": "C3"}, {"value": "-0.00522", "module": "D"}]}, "resolvedFlowVersion": "38.00.000", "flowProperties": [], "typeOfFlow": "Other flow", "classification": {"classHierarchy": "Quantities / Environmental quantities / EPD EN 15804 / LCI indicators", "name": "GaBiCategories"}}, {"dataSetInternalID": 14, "referenceToFlowDataSet": {"shortDescription": [{"value": "Components for re-use (CRU)", "lang": "en"}, {"value": "Komponenten für die Wiederverwendung (CRU)", "lang": "de"}], "type": "flow data set", "refObjectId": "a2b32f97-3fc7-4af2-b209-525bc6426f33", "uri": "../flows/a2b32f97-3fc7-4af2-b209-525bc6426f33.xml"}, "exchange direction": "OUTPUT", "other": {"anies": [{"name": "referenceToUnitGroupDataSet", "value": {"shortDescription": [{"value": "kg", "lang": "en"}], "type": "unit group data set", "refObjectId": "ad38d542-3fe9-439d-9b95-2f5f7752acaf", "uri": "../unitgroups/ad38d542-3fe9-439d-9b95-2f5f7752acaf.xml"}}, {"value": "0", "module": "A1-A3"}, {"value": "0", "module": "A4"}, {"value": "0", "module": "A5"}, {"value": "0", "module": "C3"}, {"value": "0", "module": "D"}]}, "resolvedFlowVersion": "38.00.000", "flowProperties": [], "typeOfFlow": "Other flow", "classification": {"classHierarchy": "Quantities / Environmental quantities / EPD EN 15804 / LCI indicators", "name": "GaBiCategories"}}, {"dataSetInternalID": 15, "referenceToFlowDataSet": {"shortDescription": [{"value": "Materials for recycling (MFR)", "lang": "en"}, {"value": "Stoffe zum Recycling (MFR)", "lang": "de"}], "type": "flow data set", "refObjectId": "d7fe48a5-4103-49c8-9aae-b0b5dfdbd6ae", "uri": "../flows/d7fe48a5-4103-49c8-9aae-b0b5dfdbd6ae.xml"}, "exchange direction": "OUTPUT", "other": {"anies": [{"name": "referenceToUnitGroupDataSet", "value": {"shortDescription": [{"value": "kg", "lang": "en"}], "type": "unit group data set", "refObjectId": "ad38d542-3fe9-439d-9b95-2f5f7752acaf", "uri": "../unitgroups/ad38d542-3fe9-439d-9b95-2f5f7752acaf.xml"}}, {"value": "0", "module": "A1-A3"}, {"value": "0", "module": "A4"}, {"value": "0", "module": "A5"}, {"value": "2.73", "module": "C3"}, {"value": "0", "module": "D"}]}, "resolvedFlowVersion": "38.00.000", "flowProperties": [], "typeOfFlow": "Other flow", "classification": {"classHierarchy": "Quantities / Environmental quantities / EPD EN 15804 / LCI indicators", "name": "GaBiCategories"}}, {"dataSetInternalID": 16, "referenceToFlowDataSet": {"shortDescription": [{"value": "Materials for energy recovery (MER)", "lang": "en"}, {"value": "Stoffe für die Energierückgewinnung (MER)", "lang": "de"}], "type": "flow data set", "refObjectId": "59a9181c-3aaf-46ee-8b13-2b3723b6e447", "uri": "../flows/59a9181c-3aaf-46ee-8b13-2b3723b6e447.xml"}, "exchange direction": "OUTPUT", "other": {"anies": [{"name": "referenceToUnitGroupDataSet", "value": {"shortDescription": [{"value": "kg", "lang": "en"}], "type": "unit group data set", "refObjectId": "ad38d542-3fe9-439d-9b95-2f5f7752acaf", "uri": "../unitgroups/ad38d542-3fe9-439d-9b95-2f5f7752acaf.xml"}}, {"value": "0", "module": "A1-A3"}, {"value": "0", "module": "A4"}, {"value": "0", "module": "A5"}, {"value": "0", "module": "C3"}, {"value": "0", "module": "D"}]}, "resolvedFlowVersion": "38.00.000", "flowProperties": [], "typeOfFlow": "Other flow", "classification": {"classHierarchy": "Quantities / Environmental quantities / EPD EN 15804 / LCI indicators", "name": "GaBiCategories"}}, {"dataSetInternalID": 17, "referenceToFlowDataSet": {"shortDescription": [{"value": "Exported electrical energy (EEE)", "lang": "en"}, {"value": "Exportierte elektrische Energie (EEE)", "lang": "de"}], "type": "flow data set", "refObjectId": "4da0c987-2b76-40d6-9e9e-82a017aaaf29", "uri": "../flows/4da0c987-2b76-40d6-9e9e-82a017aaaf29.xml"}, "exchange direction": "OUTPUT", "other": {"anies": [{"name": "referenceToUnitGroupDataSet", "value": {"shortDescription": [{"value": "MJ", "lang": "en"}], "type": "unit group data set", "refObjectId": "93a60a57-a3c8-11da-a746-0800200c9a66", "uri": "../unitgroups/93a60a57-a3c8-11da-a746-0800200c9a66.xml"}}, {"value": "0", "module": "A1-A3"}, {"value": "0", "module": "A4"}, {"value": "0.257", "module": "A5"}, {"value": "0.222", "module": "C3"}, {"value": "0", "module": "D"}]}, "resolvedFlowVersion": "38.00.000", "flowProperties": [], "typeOfFlow": "Other flow", "classification": {"classHierarchy": "Quantities / Environmental quantities / EPD EN 15804 / LCI indicators", "name": "GaBiCategories"}}, {"dataSetInternalID": 18, "referenceToFlowDataSet": {"shortDescription": [{"value": "Exported thermal energy (EET)", "lang": "en"}, {"value": "Exportierte thermische Energie (EET)", "lang": "de"}], "type": "flow data set", "refObjectId": "98daf38a-7a79-46d3-9a37-2b7bd0955810", "uri": "../flows/98daf38a-7a79-46d3-9a37-2b7bd0955810.xml"}, "exchange direction": "OUTPUT", "other": {"anies": [{"name": "referenceToUnitGroupDataSet", "value": {"shortDescription": [{"value": "MJ", "lang": "en"}], "type": "unit group data set", "refObjectId": "93a60a57-a3c8-11da-a746-0800200c9a66", "uri": "../unitgroups/93a60a57-a3c8-11da-a746-0800200c9a66.xml"}}, {"value": "0", "module": "A1-A3"}, {"value": "0", "module": "A4"}, {"value": "0.467", "module": "A5"}, {"value": "0.513", "module": "C3"}, {"value": "0", "module": "D"}]}, "resolvedFlowVersion": "38.00.000", "flowProperties": [], "typeOfFlow": "Other flow", "classification": {"classHierarchy": "Quantities / Environmental quantities / EPD EN 15804 / LCI indicators", "name": "GaBiCategories"}}]}, "LCIAResults": {"LCIAResult": [{"referenceToLCIAMethodDataSet": {"shortDescription": [{"value": "Global warming potential (GWP)", "lang": "en"}, {"value": "Globales Erwärmungspotenzial (GWP)", "lang": "de"}], "type": "LCIA method data set", "refObjectId": "77e416eb-a363-4258-a04e-171d843a6460", "uri": "../lciamethods/77e416eb-a363-4258-a04e-171d843a6460.xml"}, "other": {"anies": [{"name": "referenceToUnitGroupDataSet", "value": {"shortDescription": [{"value": "kg CO_(2) eq", "lang": "en"}], "type": "unit group data set", "refObjectId": "1ebf3012-d0db-4de2-aefd-ef30cedb0be1", "uri": "../unitgroups/1ebf3012-d0db-4de2-aefd-ef30cedb0be1.xml"}}, {"value": "16.3", "module": "A1-A3"}, {"value": "0.66", "module": "A4"}, {"value": "0.17", "module": "A5"}, {"value": "0.161", "module": "C3"}, {"value": "-10.3", "module": "D"}]}}, {"referenceToLCIAMethodDataSet": {"shortDescription": [{"value": "Depletion potential of the stratospheric ozone layer (ODP)", "lang": "en"}, {"value": "Abbau Potential der stratosphärischen Ozonschicht (ODP)", "lang": "de"}], "type": "LCIA method data set", "refObjectId": "06dcd26f-025f-401a-a7c1-5e457eb54637", "uri": "../lciamethods/06dcd26f-025f-401a-a7c1-5e457eb54637.xml"}, "other": {"anies": [{"name": "referenceToUnitGroupDataSet", "value": {"shortDescription": [{"value": "kg CFC11 eq", "lang": "en"}], "type": "unit group data set", "refObjectId": "88054749-b0a6-47ea-a82b-dc5b29326512", "uri": "../unitgroups/88054749-b0a6-47ea-a82b-dc5b29326512.xml"}}, {"value": "1.91E-12", "module": "A1-A3"}, {"value": "5.25E-17", "module": "A4"}, {"value": "4.09E-17", "module": "A5"}, {"value": "1.49E-16", "module": "C3"}, {"value": "7.79E-14", "module": "D"}]}}, {"referenceToLCIAMethodDataSet": {"shortDescription": [{"value": "Acidification potential of land and water (AP)", "lang": "en"}, {"value": "Versauerungspotenzial von Boden und Wasser (AP)", "lang": "de"}], "type": "LCIA method data set", "refObjectId": "b4274add-93b7-4905-a5e4-2e878c4e4216", "uri": "../lciamethods/b4274add-93b7-4905-a5e4-2e878c4e4216.xml"}, "other": {"anies": [{"name": "referenceToUnitGroupDataSet", "value": {"shortDescription": [{"value": "kg SO_(2) eq", "lang": "en"}], "type": "unit group data set", "refObjectId": "bc50c624-a9bc-45b1-a9b0-e6b10d00476f", "uri": "../unitgroups/bc50c624-a9bc-45b1-a9b0-e6b10d00476f.xml"}}, {"value": "0.0648", "module": "A1-A3"}, {"value": "0.0154", "module": "A4"}, {"value": "3.56E-05", "module": "A5"}, {"value": "5.21E-05", "module": "C3"}, {"value": "-0.0435", "module": "D"}]}}, {"referenceToLCIAMethodDataSet": {"shortDescription": [{"value": "Eutrophication potential (EP)", "lang": "en"}, {"value": "Eutrophierungspotenzial (EP)", "lang": "de"}], "type": "LCIA method data set", "refObjectId": "f58827d0-b407-4ec6-be75-8b69efb98a0f", "uri": "../lciamethods/f58827d0-b407-4ec6-be75-8b69efb98a0f.xml"}, "other": {"anies": [{"name": "referenceToUnitGroupDataSet", "value": {"shortDescription": [{"value": "kg PO_(4)^(3) eq", "lang": "en"}], "type": "unit group data set", "refObjectId": "67b5401d-873c-485f-bcf3-6ae83b918822", "uri": "../unitgroups/67b5401d-873c-485f-bcf3-6ae83b918822.xml"}}, {"value": "0.00461", "module": "A1-A3"}, {"value": "0.00174", "module": "A4"}, {"value": "6.71E-06", "module": "A5"}, {"value": "9.62E-06", "module": "C3"}, {"value": "-0.00275", "module": "D"}]}}, {"referenceToLCIAMethodDataSet": {"shortDescription": [{"value": "Formation potential of tropospheric ozone photochemical oxidants (POCP)", "lang": "en"}, {"value": "Bildungspotential für troposphärisches Ozon (POCP)", "lang": "de"}], "type": "LCIA method data set", "refObjectId": "1e84a202-dae6-42aa-9e9d-71ea48b8be00", "uri": "../lciamethods/1e84a202-dae6-42aa-9e9d-71ea48b8be00.xml"}, "other": {"anies": [{"name": "referenceToUnitGroupDataSet", "value": {"shortDescription": [{"value": "kg Ethen eq", "lang": "en"}], "type": "unit group data set", "refObjectId": "01c26c17-9a76-406e-8295-f17b55fd909e", "uri": "../unitgroups/01c26c17-9a76-406e-8295-f17b55fd909e.xml"}}, {"value": "0.00555", "module": "A1-A3"}, {"value": "0.000491", "module": "A4"}, {"value": "2.35E-06", "module": "A5"}, {"value": "3.07E-06", "module": "C3"}, {"value": "-0.0031", "module": "D"}]}}, {"referenceToLCIAMethodDataSet": {"shortDescription": [{"value": "Abiotic depletion potential for non fossil resources (ADPE)", "lang": "en"}, {"value": "Potenzial für den abiotischen Abbau nicht fossiler Ressourcen (ADPE)", "lang": "de"}], "type": "LCIA method data set", "refObjectId": "f7c73bb9-ab1a-4249-9c6d-379a0de6f67e", "uri": "../lciamethods/f7c73bb9-ab1a-4249-9c6d-379a0de6f67e.xml"}, "other": {"anies": [{"name": "referenceToUnitGroupDataSet", "value": {"shortDescription": [{"value": "kg Sb eq", "lang": "en"}], "type": "unit group data set", "refObjectId": "54ccd2d9-a32a-4fc2-923d-f2c8c93e89d4", "uri": "../unitgroups/54ccd2d9-a32a-4fc2-923d-f2c8c93e89d4.xml"}}, {"value": "0.000934", "module": "A1-A3"}, {"value": "2.18E-08", "module": "A4"}, {"value": "3.34E-09", "module": "A5"}, {"value": "2.38E-08", "module": "C3"}, {"value": "-0.000353", "module": "D"}]}}, {"referenceToLCIAMethodDataSet": {"shortDescription": [{"value": "Abiotic depletion potential for fossil resources (ADPF)", "lang": "en"}, {"value": "Potenzial für den abiotischen Abbau fossiler Brennstoffe (ADPF)", "lang": "de"}], "type": "LCIA method data set", "refObjectId": "804ebcdf-309d-4098-8ed8-fdaf2f389981", "uri": "../lciamethods/804ebcdf-309d-4098-8ed8-fdaf2f389981.xml"}, "other": {"anies": [{"name": "referenceToUnitGroupDataSet", "value": {"shortDescription": [{"value": "MJ", "lang": "en"}], "type": "unit group data set", "refObjectId": "93a60a57-a3c8-11da-a746-0800200c9a66", "uri": "../unitgroups/93a60a57-a3c8-11da-a746-0800200c9a66.xml"}}, {"value": "194", "module": "A1-A3"}, {"value": "8.62", "module": "A4"}, {"value": "0.0471", "module": "A5"}, {"value": "0.0989", "module": "C3"}, {"value": "-103", "module": "D"}]}}]}, "otherAttributes": {"{http://www.indata.network/EPD/2019}epd-version": "1.2"}, "version": "1.1", "locations": "../ILCDLocations.xml"}