{"processInformation": {"dataSetInformation": {"UUID": "7d4b035c-bc11-4c7a-befd-3eced04a30f7", "name": {"baseName": [{"value": "noraplan® 913 2 mm", "lang": "de"}, {"value": "noraplan® 913 2 mm", "lang": "en"}], "functionalUnitFlowProperties": [{"lang": "de"}]}, "classificationInformation": {"classification": [{"class": [{"value": "Kunststoffe", "level": 0, "classId": "6"}, {"value": "Bodenbeläge", "level": 1, "classId": "6.2"}, {"value": "Gummi-/Kautschuk-Bodenbeläge", "level": 2, "classId": "6.2.02"}], "name": "OEKOBAU.DAT"}, {"class": [{"value": "02 Bauprodukte", "level": 0}, {"value": "Bodenbeläge", "level": 1}, {"value": "Bodenbeläge", "level": 2}], "name": "IBUCategories"}]}, "generalComment": [{"value": "In dieser Umwelt-Produktdeklaration (EPD) werden rezepturgleiche elastische Kautschuk-Bodenbelge der Produktfamilie noraplan® 913 mit verschiedenen Designs und Oberflchenstrukturen der nora systems GmbH abgebildet.\nBesondere Merkmale der noraplan® 913 Belge sind:\n\nKontinuierlich vulkanisierte Kautschukbelge in Bahnen\n\nBelagsaufbau: Einschichtig\nOhne Zusatz von PVC, chlorhaltigen Polymeren und Phthalat-Weichmachern\nDauerelastische Eigenschaften\nGeeignet fr hchste Beanspruchungen\nKeine Beschichtungen bentigt\n\nErhhte Sicherheit wegen hoher Brandschutzeigenschaften \nUnverfugte Verlegung\nHohe Bestndigkeit gegen Chemikalien und Flchen- sowie Handdesinfektionsmittel gem den Listen von VAH und RKI", "lang": "de"}, {"value": "In this Environmental Product Declaration (EPD), resilient rubber floor coverings of the product line noraplan® 913 with different designs and surface structures are modelled. \nSpecific characteristics of the noraplan® 913 coverings are: \n\nmanufacturing method: continuously vulcanized rubber floor coverings in sheets \ncovering structure: single-layered\nno addition of PVC, chlorine-containing polymers and phthalate plasticizers\npermanently resilient\nsuitable for high traffic areas\nno coating needed\nhighly fire retardant\nno welding required \n\nhigh resistance against chemicals and surface as well as hand disinfectants according to the VAH and RKI lists", "lang": "en"}]}, "quantitativeReference": {"referenceToReferenceFlow": [0]}, "time": {"referenceYear": 2024, "dataSetValidUntil": 2029, "other": {"anies": [{"name": "publicationDateOfEPD", "value": 1733356800000}]}}, "geography": {"locationOfOperationSupplyOrProduction": {"location": "RER"}}, "technology": {"technologyDescriptionAndIncludedProcesses": [{"value": "Die Produktionsstufen sind Einwiegen, Mischen und Ausziehen der unvulkanisierten Rohlinge auf einem Kalander. Die anschließende Vulkanisation erfolgt kontinuierlich auf Fertigungslinien mit dampfbeheizten Trommel- oder Doppelbandpressen unter hohem Druck bei einer Temperatur von ca. 180°C zu 1,22 m breiten Bahnen. Nach der Vulkanisation werden die Bahnen rückseitig geschliffen und entweder als Rollenware aufgewickelt oder für Fliesenware abgelegt und gestanzt. Das Flächengewicht beträgt 3,36 kg/m². Das Qualitäts- und Energiemanagement der nora systems GmbH ist nach DIN EN ISO 9001 bzw. DIN EN ISO 50001 zertifiziert. \nTechnische Daten: \nAuszug aus technischen Datenblttern: (abrufbar auf www.nora.com) \nDeklarierte Einheit: \nAls Referenzgre wird 1 m Bodenbelag betrachtet. Die Werte des Moduls A1- A3 beziehen sich auf 1 m produziertes Produkt.\nEs handelt sich um eine Produktdeklaration. Die Herstellung und Beseitigung der Verschnitte bei der Installation werden dem Modul A5 zugeordnet. Die Module A1- A3, A4 und A5 beziehen sich gesamt auf 1 m installiertes Produkt.\nDie zur Installation notwendigen Materialien zur Vorbereitung des Untergrunds und zur Klebung werden nicht bercksichtigt. Fr den vollstndigen Bodenaufbau knnen Umweltproduktdeklarationen nach den IBU-PCR Dispersionsklebstoffe und –voranstriche sowie Mineralische Werkmrtel herangezogen werden.", "lang": "de"}, {"value": "The production stages are weighing, mixing, and stretching of the unvulcanised blanks on a calender. The following vulcanisation is continuously executed on production lines with steam heated drum or double belt presses, where under high pressure and at a temperature of approximately 180°C sheets of 1.22 m width are produced. After the vulcanising machine, the sheets are backside sanded and either wound into rolls or, for tiles, cut to length and die-cut. The mass per unit area is 3.36 kg/m². nora systems GmbH purchases the total electrical energy for production and administration at the site Weinheim from renewable energy sources. Respective evidence is available at IBU. Thermal energy is generated centrally and in heating boilers from natural gas. Our quality and energy management is certified according to DIN EN ISO 9001 and DIN EN ISO 50001. \nTechnical data: \nExcerpt of technical data sheets: (available at www.nora.com) \nDeclared unit: \nThe reference unit is 1 m of floor covering. The values of module A1-A3 refer to 1 m produced. This EPD represents a product declaration, i.e. the production and disposal of off-cuts during installation stage are assigned to module A5. The combined modules A1- A3, A4 and A5 refer to a reference unit of 1 m installed.\nThe material for subfloor preparation and adhesive bonding, needed during installation, is not considered. Information on the complete floor structure can be found in Environmental Product Declarations based to the IBU-PCR Dispersion adhesives and primers for floor coverings and Mineral factory-made mortar.", "lang": "en"}], "technologicalApplicability": [{"value": "noraplan® 913 Bodenbelge sind fr verschiedene Anwendungsbereiche geeignet, zum Beispiel fr das Gesundheits- und Bildungswesen, die Industrie und Life Science, den ffentlichen Bau sowie fr die Verwendung in Shops und Stores. Fr die Verwendung und Anwendung gelten die jeweiligen nationalen Bestimmungen.\nDie Bodenbelge werden gem DIN EN ISO 10874 klassifiziert.\nBodenbelge fr starke Beanspruchung im Objektbereich:", "lang": "de"}, {"value": "noraplan® 913 can be used in various application areas as in Healthcare, Education, Industry, Public Buildings or Shops and Stores. For use and application the respective national provisions apply.\nFloor coverings are classified according to DIN EN ISO 10874. \nFloor coverings for high performance professional use:", "lang": "en"}]}}, "modellingAndValidation": {"LCIMethodAndAllocation": {"typeOfDataSet": "EPD", "referenceToLCAMethodDetails": [{"shortDescription": [{"value": "Bodenbeläge.pdf", "lang": "de"}], "type": "source data set", "refObjectId": "46ae1eae-5f65-4b84-a6ac-9af6a11483e6"}], "other": {"anies": [{"name": "subType", "value": "specific dataset"}]}}, "dataSourcesTreatmentAndRepresentativeness": {"referenceToDataSource": [{"shortDescription": [{"value": "GaBi Database (all versions)", "lang": "de"}], "type": "source data set", "refObjectId": "28d74cc0-db8b-4d7e-bc44-5f6d56ce0c4a"}, {"shortDescription": [{"value": "Sphera MLC (fka GaBi) CUP 2023.02", "lang": "de"}], "type": "source data set", "refObjectId": "cb600d3b-e85a-42b3-b059-5591e2757fbb"}], "useAdviceForDataSet": [{"value": "Gültigkeitsbereich: \nProduktfamilie noraplan® 913 mit einer Dicke von 2 mm.Kontinuierlich in Bahnen vulkanisierte Bodenbelge aus Kautschuk in verschiedenen Farben und Designs. Diese Deklaration ist eine Umweltproduktdeklaration gem ISO 14025 und beschreibt die spezifische Umweltleistung der hier genannten Bauprodukte in Deutschland am Produktionsstandort Weinheim (Bergstrae). \nSystemgrenze: \nTyp der EPD: von der Wiege bis zum Werkstor mit Optionen.\nDie kobilanzielle Berechnung umfasst folgende\nPhasen:\nHerstellungsphase A1- A3: Bercksichtigung der Vorkette und der Produktion des\nBodenbelags, inkl. Verpackung (Input von Altpapier bei der Papier-/Kartonherstellung).\nTransport A4: Annahme fr den Transport der Produkte zur Baustelle.\nInstallationsphase A5: Bercksichtigung der Herstellung und des Transports der Verschnitt Menge, Verbrennung des Verschnitts (gewonnene Energie wird in D als vermiedene Umweltlasten deklariert), Entsorgung der Verpackungsmaterialien (Verbrennung der Polyethylenfolie). Die Untergrundvorbehandlung (Grundierung, Spachtelmasse, Klebstoff) bleibt unbercksichtigt. Diese ist abhngig vom Gebude und der Anwendung und muss im\nEinzelfall spezifiziert werden.\nNutzungsphase B2: Szenario fr die Reinigung entsprechend den Herstellerempfehlungen (siehe 4.).\nEnd-of-Life-Phase C1, C2, C3: Szenario fr die Verbrennung des Bodenbelags inkl.\nAusbau aus dem Gebude und Transport zum Verbrennungsort (gewonnene Energie\nwird in D als vermiedene Umweltlasten deklariert). Modul C4 wird mit 0 deklariert, da das EOL-Szenario keine Deponierung beinhaltet.\nNutzen und Lasten fr das nchste System D: Gewinnung von elektrischer und thermischer\nEnergie aus der thermischen Verwertung des Produkts, des Installationsverschnitts und der\nVerpackung Einflsse von Abfllen werden in den Modulen bercksichtigt, in denen diese anfallen.\nFr die Umweltauswirkungen wurde der Einsatz von grnem Strom unter Bercksichtigung des Reststrommixes fr den brigen Strom berechnet. Der Anteil des mit grnem Strom gedeckten Strombedarfs am Gesamtstrombedarf betrgt 100 %.", "lang": "de"}, {"value": "Scope: \nProduct line noraplan® 913 with a thickness of 2 mm. \nRubber floor coverings continuously vulcanised in sheets in various colours and designs.\nThis declaration is an Environmental Product Declaration according to ISO 14025 describing the specific environmental performance of the mentioned construction products produced in Weinheim/Bergstrae Germany. \nSystem boundary: \nType of EPD: from cradle to gate with options.\nThe analysis of the product life cycle includes the following stages:\nProduction stage A1-A3: Consideration of production of the basic materials and the manufacturing of the floor covering incl. packaging material (input of waste paper forpaper/cardboard production).\nTransport A4: Assumption for the transport of the products to the construction site.\nInstallation A5: Production, transport and incineration of the off-cut material, incineration of off-cut material (gained energy is declared in D as avoided environmental burden), disposal of the packaging (incineration of PE film). The pretreatment of the underground surface (prime coat, levelling compound, adhesive) is not considered. This treatment depends on the building and the application and need to be specified for the particular case.\nUse stage B2: Scenario for maintenance/cleaning according to the manufacturers recommendation (see 4.)\nEnd-of-Life stage C1, C2, C3: Scenario for the incineration of the floor covering incl. removal from the building and transport to the waste incineration plant (gained energy is declared in D as avoided environmental burden). Module C4 is declared 0 because the EOL scenario does not include landfilling.\nBenefits for the next product system D: Extraction for electrical and thermal energy from the waste incineration process of the product, the off-cuts and the packaging material.Contributions of waste flows are considered in the modules where they occur.\nFor the environmental impact, the use of green electricity was calculated taking into account the residual electricity mix for the remaining electricity. The proportion of the total electricity requirement covered by green electricity is 100%.", "lang": "en"}], "other": {"anies": [{"name": "referenceToOriginalEPD", "value": {"shortDescription": {"value": "noraplan® 913 2 mm.pdf", "defaultValue": "noraplan® 913 2 mm.pdf", "lstrings": [{"lang": "de", "value": "noraplan® 913 2 mm.pdf"}]}, "type": "source data set", "uuid": {"uuid": "502a8027-bc7c-4eab-a52d-b627fd562af6"}, "refObjectId": "502a8027-bc7c-4eab-a52d-b627fd562af6", "resourceURLs": ["https://oekobaudat.de/OEKOBAU.DAT/resource/sources/502a8027-bc7c-4eab-a52d-b627fd562af6/noraplan_913_2_mm_19120.pdf?version=00.01.000"]}}]}}, "validation": {"review": [{"referenceToNameOfReviewerAndInstitution": [{"shortDescription": [{"value": "Institut Bauen und Umwelt e. V.", "lang": "de"}], "type": "contact data set", "refObjectId": "d111dbec-b024-4be5-86c5-752d6eb2cf95", "uri": "../contacts/d111dbec-b024-4be5-86c5-752d6eb2cf95.xml"}], "type": "Accredited third party review"}]}, "complianceDeclarations": {"compliance": [{"referenceToComplianceSystem": {"shortDescription": [{"value": "DIN EN 15804+A2", "lang": "de"}], "type": "source data set", "refObjectId": "c0016b33-8cf7-415c-ac6e-deba0d21440d", "uri": "../sources/c0016b33-8cf7-415c-ac6e-deba0d21440d.xml"}}, {"referenceToComplianceSystem": {"shortDescription": [{"value": "ISO 14025", "lang": "de"}], "type": "source data set", "refObjectId": "4f2eb655-6e44-4874-a95a-e28f5442cd4d", "uri": "../sources/4f2eb655-6e44-4874-a95a-e28f5442cd4d.xml"}}]}}, "administrativeInformation": {"commissionerAndGoal": {"referenceToCommissioner": [{"shortDescription": [{"value": "nora systems GmbH", "lang": "de"}], "type": "contact data set", "refObjectId": "6116f444-2f51-49a2-8f7e-82c2cbb7f3ff", "uri": "../contacts/6116f444-2f51-49a2-8f7e-82c2cbb7f3ff.xml"}]}, "dataGenerator": {"referenceToPersonOrEntityGeneratingTheDataSet": [{"shortDescription": [{"value": "Angela Schindler Umweltberatung", "lang": "de"}], "type": "contact data set", "refObjectId": "2d08611b-4b49-488c-815b-e516828eed87", "uri": "../contacts/2d08611b-4b49-488c-815b-e516828eed87.xml"}]}, "dataEntryBy": {"timeStamp": 1733356800000, "referenceToDataSetFormat": [{"shortDescription": [{"value": "ILCD Format", "lang": "de"}], "type": "source data set", "refObjectId": "a97a0155-0234-4b87-b4ce-a45da52f2a40", "uri": "../sources/a97a0155-0234-4b87-b4ce-a45da52f2a40.xml"}, {"shortDescription": [{"value": "EPD-Datenformaterweiterungen v1.2", "lang": "de"}, {"value": "EPD Data Format Extensions v1.2", "lang": "en"}], "type": "source data set", "refObjectId": "a29449fd-aa2f-4de8-b5d7-4b06b43c6fde", "uri": "../sources/a29449fd-aa2f-4de8-b5d7-4b06b43c6fde.xml"}]}, "publicationAndOwnership": {"dataSetVersion": "00.02.000", "referenceToPrecedingDataSetVersion": [{"shortDescription": [{"value": "noraplan® 913", "lang": "de"}], "type": "process data set", "refObjectId": "eec4acca-9f3c-4628-8298-9c53875034cf", "uri": "../processes/eec4acca-9f3c-4628-8298-9c53875034cf.xml"}], "referenceToRegistrationAuthority": {"shortDescription": [{"value": "Institut Bauen und Umwelt e. V.", "lang": "de"}], "type": "contact data set", "refObjectId": "d111dbec-b024-4be5-86c5-752d6eb2cf95", "uri": "../contacts/d111dbec-b024-4be5-86c5-752d6eb2cf95.xml"}, "registrationNumber": "EPD-NOR-20240470-IBA1-DE", "referenceToOwnershipOfDataSet": {"shortDescription": [{"value": "nora systems GmbH", "lang": "de"}], "type": "contact data set", "refObjectId": "6116f444-2f51-49a2-8f7e-82c2cbb7f3ff", "uri": "../contacts/6116f444-2f51-49a2-8f7e-82c2cbb7f3ff.xml"}, "copyright": true, "licenseType": "Free of charge for all users and uses", "accessRestrictions": [{"value": "None", "lang": "en"}], "other": {"anies": [{"name": "referenceToPublisher", "value": {"shortDescription": [{"value": "Institut Bauen und Umwelt e. V.", "lang": "de"}], "type": "contact data set", "refObjectId": "d111dbec-b024-4be5-86c5-752d6eb2cf95", "uri": "../contacts/d111dbec-b024-4be5-86c5-752d6eb2cf95.xml"}}]}}}, "exchanges": {"exchange": [{"dataSetInternalID": 0, "referenceToFlowDataSet": {"shortDescription": [{"value": "noraplan® 913/ 1 m2 (noraplan® 913/ 1 m2)", "lang": "de"}], "type": "flow data set", "refObjectId": "f76b95cf-4ede-c286-a5a9-d9e0dbea9887", "uri": "../flows/f76b95cf-4ede-c286-a5a9-d9e0dbea9887.xml"}, "meanAmount": 1.0, "referencesToDataSource": {}, "referenceFlow": true, "resolvedFlowVersion": "00.03.000", "resultingflowAmount": 1.0, "flowProperties": [{"name": [{"lang": "de", "value": "Fläche"}, {"lang": "en", "value": "Area"}], "uuid": "93a60a56-a3c8-19da-a746-0800200c9a66", "referenceFlowProperty": true, "meanValue": 1.0, "referenceUnit": "qm", "unitGroupUUID": "c20a03d7-bd90-4569-bc94-66cfd364dfc8"}], "materialProperties": [{"name": "grammage", "value": "3.36", "unit": "kg/m^2", "unitDescription": "kilograms per square meter"}, {"name": "gross density", "value": "3.36", "unit": "kg/m^3", "unitDescription": "kilograms per cubic metre"}, {"name": "layer thickness", "value": "0.002", "unit": "m", "unitDescription": "meters"}], "typeOfFlow": "Product flow", "classification": {"classHierarchy": "Kunststoffe / Bodenbeläge / Gummi-/Kautschuk-Bodenbeläge", "name": "OEKOBAU.DAT"}}, {"dataSetInternalID": 1, "referenceToFlowDataSet": {"shortDescription": [{"value": "Erneuerbare Primärenergie als Energieträger (PERE)", "lang": "de"}, {"value": "Renewable primary energy as energy carrier (PERE)", "lang": "en"}], "type": "flow data set", "refObjectId": "20f32be5-0398-4288-9b6d-accddd195317", "uri": "../flows/20f32be5-0398-4288-9b6d-accddd195317.xml"}, "exchange direction": "INPUT", "other": {"anies": [{"name": "referenceToUnitGroupDataSet", "value": {"shortDescription": [{"value": "MJ", "lang": "de"}], "type": "unit group data set", "refObjectId": "93a60a57-a3c8-11da-a746-0800200c9a66", "uri": "../unitgroups/93a60a57-a3c8-11da-a746-0800200c9a66.xml"}}, {"value": "16.6854004897957", "module": "A1-A3"}, {"value": "0.197954375904307", "module": "A4"}, {"value": "1.86047235071826", "module": "A5"}, {"value": "0.107034723276037", "module": "B2"}, {"value": "0.405820076487879", "module": "C1"}, {"value": "0.00981698936936664", "module": "C2"}, {"value": "17.1309892290262", "module": "C3"}, {"value": "0", "module": "C4"}, {"value": "-4.56511787819034", "module": "D"}]}, "resolvedFlowVersion": "38.00.000", "flowProperties": [], "typeOfFlow": "Other flow", "classification": {"classHierarchy": "Quantities", "name": "GaBiCategories"}}, {"dataSetInternalID": 2, "referenceToFlowDataSet": {"shortDescription": [{"value": "Erneuerbare Primärenergie zur stofflichen Nutzung (PERM)", "lang": "de"}, {"value": "Renewable primary energy resources as material utilization (PERM)", "lang": "en"}], "type": "flow data set", "refObjectId": "fb3ec0de-548d-4508-aea5-00b73bf6f702", "uri": "../flows/fb3ec0de-548d-4508-aea5-00b73bf6f702.xml"}, "exchange direction": "INPUT", "other": {"anies": [{"name": "referenceToUnitGroupDataSet", "value": {"shortDescription": [{"value": "MJ", "lang": "de"}], "type": "unit group data set", "refObjectId": "93a60a57-a3c8-11da-a746-0800200c9a66", "uri": "../unitgroups/93a60a57-a3c8-11da-a746-0800200c9a66.xml"}}, {"value": "17.15208", "module": "A1-A3"}, {"value": "0", "module": "A4"}, {"value": "-0.1236", "module": "A5"}, {"value": "0", "module": "B2"}, {"value": "0", "module": "C1"}, {"value": "0", "module": "C2"}, {"value": "-17.02848", "module": "C3"}, {"value": "0", "module": "C4"}, {"value": "0", "module": "D"}]}, "resolvedFlowVersion": "38.00.000", "flowProperties": [], "typeOfFlow": "Other flow", "classification": {"classHierarchy": "Quantities", "name": "GaBiCategories"}}, {"dataSetInternalID": 3, "referenceToFlowDataSet": {"shortDescription": [{"value": "Total erneuerbare Primärenergie (PERT)", "lang": "de"}, {"value": "Total use of renewable primary energy resources (PERT)", "lang": "en"}], "type": "flow data set", "refObjectId": "53f97275-fa8a-4cdd-9024-65936002acd0", "uri": "../flows/53f97275-fa8a-4cdd-9024-65936002acd0.xml"}, "exchange direction": "INPUT", "other": {"anies": [{"name": "referenceToUnitGroupDataSet", "value": {"shortDescription": [{"value": "MJ", "lang": "de"}], "type": "unit group data set", "refObjectId": "93a60a57-a3c8-11da-a746-0800200c9a66", "uri": "../unitgroups/93a60a57-a3c8-11da-a746-0800200c9a66.xml"}}, {"value": "33.8374804897957", "module": "A1-A3"}, {"value": "0.197954375904307", "module": "A4"}, {"value": "1.73687235071826", "module": "A5"}, {"value": "0.107034723276037", "module": "B2"}, {"value": "0.405820076487879", "module": "C1"}, {"value": "0.00981698936936664", "module": "C2"}, {"value": "0.102509229026247", "module": "C3"}, {"value": "0", "module": "C4"}, {"value": "-4.56511787819034", "module": "D"}]}, "resolvedFlowVersion": "38.00.000", "flowProperties": [], "typeOfFlow": "Other flow", "classification": {"classHierarchy": "Quantities / Environmental quantities / EPD EN 15804 / LCI indicators", "name": "GaBiCategories"}}, {"dataSetInternalID": 4, "referenceToFlowDataSet": {"shortDescription": [{"value": "Nicht-erneuerbare Primärenergie als Energieträger (PENRE)", "lang": "de"}, {"value": "Non renewable primary energy as energy carrier (PENRE)", "lang": "en"}], "type": "flow data set", "refObjectId": "ac857178-2b45-46ec-892a-a9a4332f0372", "uri": "../flows/ac857178-2b45-46ec-892a-a9a4332f0372.xml"}, "exchange direction": "INPUT", "other": {"anies": [{"name": "referenceToUnitGroupDataSet", "value": {"shortDescription": [{"value": "MJ", "lang": "de"}], "type": "unit group data set", "refObjectId": "93a60a57-a3c8-11da-a746-0800200c9a66", "uri": "../unitgroups/93a60a57-a3c8-11da-a746-0800200c9a66.xml"}}, {"value": "85.8939910000356", "module": "A1-A3"}, {"value": "3.07504599574131", "module": "A4"}, {"value": "5.87064655026222", "module": "A5"}, {"value": "2.32549438794639", "module": "B2"}, {"value": "0.679049388606871", "module": "C1"}, {"value": "0.135406242305128", "module": "C2"}, {"value": "24.5890783386632", "module": "C3"}, {"value": "0", "module": "C4"}, {"value": "-15.6338011359302", "module": "D"}]}, "resolvedFlowVersion": "38.00.000", "flowProperties": [], "typeOfFlow": "Other flow", "classification": {"classHierarchy": "Quantities", "name": "GaBiCategories"}}, {"dataSetInternalID": 5, "referenceToFlowDataSet": {"shortDescription": [{"value": "Nicht-erneuerbare Primärenergie zur stofflichen Nutzung (PENRM)", "lang": "de"}, {"value": "Non renewable primary energy as material utilization (PENRM)", "lang": "en"}], "type": "flow data set", "refObjectId": "1421caa0-679d-4bf4-b282-0eb850ccae27", "uri": "../flows/1421caa0-679d-4bf4-b282-0eb850ccae27.xml"}, "exchange direction": "INPUT", "other": {"anies": [{"name": "referenceToUnitGroupDataSet", "value": {"shortDescription": [{"value": "MJ", "lang": "de"}], "type": "unit group data set", "refObjectId": "93a60a57-a3c8-11da-a746-0800200c9a66", "uri": "../unitgroups/93a60a57-a3c8-11da-a746-0800200c9a66.xml"}}, {"value": "24.276976", "module": "A1-A3"}, {"value": "0", "module": "A4"}, {"value": "-0.088", "module": "A5"}, {"value": "0", "module": "B2"}, {"value": "0", "module": "C1"}, {"value": "0", "module": "C2"}, {"value": "-24.188976", "module": "C3"}, {"value": "0", "module": "C4"}, {"value": "0", "module": "D"}]}, "resolvedFlowVersion": "38.00.000", "flowProperties": [], "typeOfFlow": "Other flow", "classification": {"classHierarchy": "Quantities", "name": "GaBiCategories"}}, {"dataSetInternalID": 6, "referenceToFlowDataSet": {"shortDescription": [{"value": "Total nicht erneuerbare Primärenergie (PENRT)", "lang": "de"}, {"value": "Total use of non renewable primary energy resources (PENRT)", "lang": "en"}], "type": "flow data set", "refObjectId": "06159210-646b-4c8d-8583-da9b3b95a6c1", "uri": "../flows/06159210-646b-4c8d-8583-da9b3b95a6c1.xml"}, "exchange direction": "INPUT", "other": {"anies": [{"name": "referenceToUnitGroupDataSet", "value": {"shortDescription": [{"value": "MJ", "lang": "de"}], "type": "unit group data set", "refObjectId": "93a60a57-a3c8-11da-a746-0800200c9a66", "uri": "../unitgroups/93a60a57-a3c8-11da-a746-0800200c9a66.xml"}}, {"value": "110.170967000036", "module": "A1-A3"}, {"value": "3.07504599574131", "module": "A4"}, {"value": "5.78264655026222", "module": "A5"}, {"value": "2.32549438794639", "module": "B2"}, {"value": "0.679049388606871", "module": "C1"}, {"value": "0.135406242305128", "module": "C2"}, {"value": "0.40010233866319", "module": "C3"}, {"value": "0", "module": "C4"}, {"value": "-15.6338011359302", "module": "D"}]}, "resolvedFlowVersion": "38.00.000", "flowProperties": [], "typeOfFlow": "Other flow", "classification": {"classHierarchy": "Quantities / Environmental quantities / EPD EN 15804 / LCI indicators", "name": "GaBiCategories"}}, {"dataSetInternalID": 7, "referenceToFlowDataSet": {"shortDescription": [{"value": "Einsatz von Sekundärstoffen (SM)", "lang": "de"}, {"value": "Use of secondary material (SM)", "lang": "en"}], "type": "flow data set", "refObjectId": "c6a1f35f-2d09-4f54-8dfb-97e502e1ce92", "uri": "../flows/c6a1f35f-2d09-4f54-8dfb-97e502e1ce92.xml"}, "exchange direction": "INPUT", "other": {"anies": [{"name": "referenceToUnitGroupDataSet", "value": {"shortDescription": [{"value": "kg", "lang": "de"}], "type": "unit group data set", "refObjectId": "ad38d542-3fe9-439d-9b95-2f5f7752acaf", "uri": "../unitgroups/ad38d542-3fe9-439d-9b95-2f5f7752acaf.xml"}}, {"value": "0.026", "module": "A1-A3"}, {"value": "0", "module": "A4"}, {"value": "0", "module": "A5"}, {"value": "0", "module": "B2"}, {"value": "0", "module": "C1"}, {"value": "0", "module": "C2"}, {"value": "0", "module": "C3"}, {"value": "0", "module": "C4"}, {"value": "0", "module": "D"}]}, "resolvedFlowVersion": "38.00.000", "flowProperties": [], "typeOfFlow": "Other flow", "classification": {"classHierarchy": "Quantities / Environmental quantities / EPD EN 15804 / LCI indicators", "name": "GaBiCategories"}}, {"dataSetInternalID": 8, "referenceToFlowDataSet": {"shortDescription": [{"value": "Erneuerbare Sekundärbrennstoffe (RSF)", "lang": "de"}, {"value": "Use of renewable secondary fuels (RSF)", "lang": "en"}], "type": "flow data set", "refObjectId": "64333088-a55f-4aa2-9a31-c10b07816787", "uri": "../flows/64333088-a55f-4aa2-9a31-c10b07816787.xml"}, "exchange direction": "INPUT", "other": {"anies": [{"name": "referenceToUnitGroupDataSet", "value": {"shortDescription": [{"value": "MJ", "lang": "de"}], "type": "unit group data set", "refObjectId": "93a60a57-a3c8-11da-a746-0800200c9a66", "uri": "../unitgroups/93a60a57-a3c8-11da-a746-0800200c9a66.xml"}}, {"value": "0", "module": "A1-A3"}, {"value": "0", "module": "A4"}, {"value": "0", "module": "A5"}, {"value": "0", "module": "B2"}, {"value": "0", "module": "C1"}, {"value": "0", "module": "C2"}, {"value": "0", "module": "C3"}, {"value": "0", "module": "C4"}, {"value": "0", "module": "D"}]}, "resolvedFlowVersion": "38.00.000", "flowProperties": [], "typeOfFlow": "Other flow", "classification": {"classHierarchy": "Quantities / Environmental quantities / EPD EN 15804 / LCI indicators", "name": "GaBiCategories"}}, {"dataSetInternalID": 9, "referenceToFlowDataSet": {"shortDescription": [{"value": "Nicht erneuerbare Sekundärbrennstoffe (NRSF)", "lang": "de"}, {"value": "Use of non renewable secondary fuels (NRSF)", "lang": "en"}], "type": "flow data set", "refObjectId": "89def144-d39a-4287-b86f-efde453ddcb2", "uri": "../flows/89def144-d39a-4287-b86f-efde453ddcb2.xml"}, "exchange direction": "INPUT", "other": {"anies": [{"name": "referenceToUnitGroupDataSet", "value": {"shortDescription": [{"value": "MJ", "lang": "de"}], "type": "unit group data set", "refObjectId": "93a60a57-a3c8-11da-a746-0800200c9a66", "uri": "../unitgroups/93a60a57-a3c8-11da-a746-0800200c9a66.xml"}}, {"value": "0", "module": "A1-A3"}, {"value": "0", "module": "A4"}, {"value": "0", "module": "A5"}, {"value": "0", "module": "B2"}, {"value": "0", "module": "C1"}, {"value": "0", "module": "C2"}, {"value": "0", "module": "C3"}, {"value": "0", "module": "C4"}, {"value": "0", "module": "D"}]}, "resolvedFlowVersion": "38.00.000", "flowProperties": [], "typeOfFlow": "Other flow", "classification": {"classHierarchy": "Quantities / Environmental quantities / EPD EN 15804 / LCI indicators", "name": "GaBiCategories"}}, {"dataSetInternalID": 10, "referenceToFlowDataSet": {"shortDescription": [{"value": "Einsatz von Süßwasserressourcen (FW)", "lang": "de"}, {"value": "Use of net fresh water (FW)", "lang": "en"}], "type": "flow data set", "refObjectId": "3cf952c8-f3a4-461d-8c96-96456ca62246", "uri": "../flows/3cf952c8-f3a4-461d-8c96-96456ca62246.xml"}, "exchange direction": "INPUT", "other": {"anies": [{"name": "referenceToUnitGroupDataSet", "value": {"shortDescription": [{"value": "m^3", "lang": "de"}], "type": "unit group data set", "refObjectId": "cd950537-0a98-4044-9ba7-9f9a68d0a504", "uri": "../unitgroups/cd950537-0a98-4044-9ba7-9f9a68d0a504.xml"}}, {"value": "1.54853117810814", "module": "A1-A3"}, {"value": "0.0002171721091114", "module": "A4"}, {"value": "0.0790585008679665", "module": "A5"}, {"value": "0.00039246748669243", "module": "B2"}, {"value": "0.000327646301193307", "module": "C1"}, {"value": "1.07522492065713E-05", "module": "C2"}, {"value": "0.00502455712542214", "module": "C3"}, {"value": "0", "module": "C4"}, {"value": "-0.00369865304645537", "module": "D"}]}, "resolvedFlowVersion": "38.00.000", "flowProperties": [], "typeOfFlow": "Other flow", "classification": {"classHierarchy": "Quantities / Environmental quantities / EPD EN 15804 / LCI indicators", "name": "GaBiCategories"}}, {"dataSetInternalID": 11, "referenceToFlowDataSet": {"shortDescription": [{"value": "Gefährlicher Abfall zur Deponie (HWD)", "lang": "de"}, {"value": "Hazardous waste disposed (HWD)", "lang": "en"}], "type": "flow data set", "refObjectId": "430f9e0f-59b2-46a0-8e0d-55e0e84948fc", "uri": "../flows/430f9e0f-59b2-46a0-8e0d-55e0e84948fc.xml"}, "exchange direction": "OUTPUT", "other": {"anies": [{"name": "referenceToUnitGroupDataSet", "value": {"shortDescription": [{"value": "kg", "lang": "de"}], "type": "unit group data set", "refObjectId": "ad38d542-3fe9-439d-9b95-2f5f7752acaf", "uri": "../unitgroups/ad38d542-3fe9-439d-9b95-2f5f7752acaf.xml"}}, {"value": "8.75475988908928E-06", "module": "A1-A3"}, {"value": "9.56081438250885E-12", "module": "A4"}, {"value": "4.45194139177367E-07", "module": "A5"}, {"value": "0.000123702728485865", "module": "B2"}, {"value": "-5.31316657007104E-11", "module": "C1"}, {"value": "4.19260697445123E-13", "module": "C2"}, {"value": "7.10235377056775E-12", "module": "C3"}, {"value": "0", "module": "C4"}, {"value": "-8.25015599672538E-10", "module": "D"}]}, "resolvedFlowVersion": "38.00.000", "flowProperties": [], "typeOfFlow": "Other flow", "classification": {"classHierarchy": "Quantities / Environmental quantities / EPD EN 15804 / LCI indicators", "name": "GaBiCategories"}}, {"dataSetInternalID": 12, "referenceToFlowDataSet": {"shortDescription": [{"value": "Entsorgter nicht gefährlicher Abfall (NHWD)", "lang": "de"}, {"value": "Non hazardous waste disposed (NHWD)", "lang": "en"}], "type": "flow data set", "refObjectId": "b29ef66b-e286-4afa-949f-62f1a7b4d7fa", "uri": "../flows/b29ef66b-e286-4afa-949f-62f1a7b4d7fa.xml"}, "exchange direction": "OUTPUT", "other": {"anies": [{"name": "referenceToUnitGroupDataSet", "value": {"shortDescription": [{"value": "kg", "lang": "de"}], "type": "unit group data set", "refObjectId": "ad38d542-3fe9-439d-9b95-2f5f7752acaf", "uri": "../unitgroups/ad38d542-3fe9-439d-9b95-2f5f7752acaf.xml"}}, {"value": "2.37022198847689", "module": "A1-A3"}, {"value": "0.000446390951796149", "module": "A4"}, {"value": "0.124798727749695", "module": "A5"}, {"value": "0.00892204323308019", "module": "B2"}, {"value": "0.000497307497764054", "module": "C1"}, {"value": "2.06412122424442E-05", "module": "C2"}, {"value": "0.0750350013293676", "module": "C3"}, {"value": "0", "module": "C4"}, {"value": "-0.00773282880567942", "module": "D"}]}, "resolvedFlowVersion": "38.00.000", "flowProperties": [], "typeOfFlow": "Other flow", "classification": {"classHierarchy": "Quantities / Environmental quantities / EPD EN 15804 / LCI indicators", "name": "GaBiCategories"}}, {"dataSetInternalID": 13, "referenceToFlowDataSet": {"shortDescription": [{"value": "Entsorgter radioaktiver Abfall (RWD)", "lang": "de"}, {"value": "Radioactive waste disposed (RWD)", "lang": "en"}], "type": "flow data set", "refObjectId": "3449546e-52ad-4b39-b809-9fb77cea8ff6", "uri": "../flows/3449546e-52ad-4b39-b809-9fb77cea8ff6.xml"}, "exchange direction": "OUTPUT", "other": {"anies": [{"name": "referenceToUnitGroupDataSet", "value": {"shortDescription": [{"value": "kg", "lang": "de"}], "type": "unit group data set", "refObjectId": "ad38d542-3fe9-439d-9b95-2f5f7752acaf", "uri": "../unitgroups/ad38d542-3fe9-439d-9b95-2f5f7752acaf.xml"}}, {"value": "0.00119873247321919", "module": "A1-A3"}, {"value": "5.50287689803649E-06", "module": "A4"}, {"value": "6.25878909073168E-05", "module": "A5"}, {"value": "4.89417927542667E-05", "module": "B2"}, {"value": "0.000107941069402033", "module": "C1"}, {"value": "2.53404728742343E-07", "module": "C2"}, {"value": "2.25473586708415E-05", "module": "C3"}, {"value": "0", "module": "C4"}, {"value": "-0.00121141145732184", "module": "D"}]}, "resolvedFlowVersion": "38.00.000", "flowProperties": [], "typeOfFlow": "Other flow", "classification": {"classHierarchy": "Quantities / Environmental quantities / EPD EN 15804 / LCI indicators", "name": "GaBiCategories"}}, {"dataSetInternalID": 14, "referenceToFlowDataSet": {"shortDescription": [{"value": "Komponenten für die Wiederverwendung (CRU)", "lang": "de"}, {"value": "Components for re-use (CRU)", "lang": "en"}], "type": "flow data set", "refObjectId": "a2b32f97-3fc7-4af2-b209-525bc6426f33", "uri": "../flows/a2b32f97-3fc7-4af2-b209-525bc6426f33.xml"}, "exchange direction": "OUTPUT", "other": {"anies": [{"name": "referenceToUnitGroupDataSet", "value": {"shortDescription": [{"value": "kg", "lang": "de"}], "type": "unit group data set", "refObjectId": "ad38d542-3fe9-439d-9b95-2f5f7752acaf", "uri": "../unitgroups/ad38d542-3fe9-439d-9b95-2f5f7752acaf.xml"}}, {"value": "0", "module": "A1-A3"}, {"value": "0", "module": "A4"}, {"value": "0", "module": "A5"}, {"value": "0", "module": "B2"}, {"value": "0", "module": "C1"}, {"value": "0", "module": "C2"}, {"value": "0", "module": "C3"}, {"value": "0", "module": "C4"}, {"value": "0", "module": "D"}]}, "resolvedFlowVersion": "38.00.000", "flowProperties": [], "typeOfFlow": "Other flow", "classification": {"classHierarchy": "Quantities / Environmental quantities / EPD EN 15804 / LCI indicators", "name": "GaBiCategories"}}, {"dataSetInternalID": 15, "referenceToFlowDataSet": {"shortDescription": [{"value": "Stoffe zum Recycling (MFR)", "lang": "de"}, {"value": "Materials for recycling (MFR)", "lang": "en"}], "type": "flow data set", "refObjectId": "d7fe48a5-4103-49c8-9aae-b0b5dfdbd6ae", "uri": "../flows/d7fe48a5-4103-49c8-9aae-b0b5dfdbd6ae.xml"}, "exchange direction": "OUTPUT", "other": {"anies": [{"name": "referenceToUnitGroupDataSet", "value": {"shortDescription": [{"value": "kg", "lang": "de"}], "type": "unit group data set", "refObjectId": "ad38d542-3fe9-439d-9b95-2f5f7752acaf", "uri": "../unitgroups/ad38d542-3fe9-439d-9b95-2f5f7752acaf.xml"}}, {"value": "0", "module": "A1-A3"}, {"value": "0", "module": "A4"}, {"value": "0", "module": "A5"}, {"value": "0", "module": "B2"}, {"value": "0", "module": "C1"}, {"value": "0", "module": "C2"}, {"value": "0", "module": "C3"}, {"value": "0", "module": "C4"}, {"value": "0", "module": "D"}]}, "resolvedFlowVersion": "38.00.000", "flowProperties": [], "typeOfFlow": "Other flow", "classification": {"classHierarchy": "Quantities / Environmental quantities / EPD EN 15804 / LCI indicators", "name": "GaBiCategories"}}, {"dataSetInternalID": 16, "referenceToFlowDataSet": {"shortDescription": [{"value": "Stoffe für die Energierückgewinnung (MER)", "lang": "de"}, {"value": "Materials for energy recovery (MER)", "lang": "en"}], "type": "flow data set", "refObjectId": "59a9181c-3aaf-46ee-8b13-2b3723b6e447", "uri": "../flows/59a9181c-3aaf-46ee-8b13-2b3723b6e447.xml"}, "exchange direction": "OUTPUT", "other": {"anies": [{"name": "referenceToUnitGroupDataSet", "value": {"shortDescription": [{"value": "kg", "lang": "de"}], "type": "unit group data set", "refObjectId": "ad38d542-3fe9-439d-9b95-2f5f7752acaf", "uri": "../unitgroups/ad38d542-3fe9-439d-9b95-2f5f7752acaf.xml"}}, {"value": "0", "module": "A1-A3"}, {"value": "0", "module": "A4"}, {"value": "0", "module": "A5"}, {"value": "0", "module": "B2"}, {"value": "0", "module": "C1"}, {"value": "0", "module": "C2"}, {"value": "0", "module": "C3"}, {"value": "0", "module": "C4"}, {"value": "0", "module": "D"}]}, "resolvedFlowVersion": "38.00.000", "flowProperties": [], "typeOfFlow": "Other flow", "classification": {"classHierarchy": "Quantities / Environmental quantities / EPD EN 15804 / LCI indicators", "name": "GaBiCategories"}}, {"dataSetInternalID": 17, "referenceToFlowDataSet": {"shortDescription": [{"value": "Exportierte elektrische Energie (EEE)", "lang": "de"}, {"value": "Exported electrical energy (EEE)", "lang": "en"}], "type": "flow data set", "refObjectId": "4da0c987-2b76-40d6-9e9e-82a017aaaf29", "uri": "../flows/4da0c987-2b76-40d6-9e9e-82a017aaaf29.xml"}, "exchange direction": "OUTPUT", "other": {"anies": [{"name": "referenceToUnitGroupDataSet", "value": {"shortDescription": [{"value": "MJ", "lang": "de"}], "type": "unit group data set", "refObjectId": "93a60a57-a3c8-11da-a746-0800200c9a66", "uri": "../unitgroups/93a60a57-a3c8-11da-a746-0800200c9a66.xml"}}, {"value": "0", "module": "A1-A3"}, {"value": "0", "module": "A4"}, {"value": "0.0199710683495579", "module": "A5"}, {"value": "0", "module": "B2"}, {"value": "0", "module": "C1"}, {"value": "0", "module": "C2"}, {"value": "3.79794098050736", "module": "C3"}, {"value": "0", "module": "C4"}, {"value": "0", "module": "D"}]}, "resolvedFlowVersion": "38.00.000", "flowProperties": [], "typeOfFlow": "Other flow", "classification": {"classHierarchy": "Quantities / Environmental quantities / EPD EN 15804 / LCI indicators", "name": "GaBiCategories"}}, {"dataSetInternalID": 18, "referenceToFlowDataSet": {"shortDescription": [{"value": "Exportierte thermische Energie (EET)", "lang": "de"}, {"value": "Exported thermal energy (EET)", "lang": "en"}], "type": "flow data set", "refObjectId": "98daf38a-7a79-46d3-9a37-2b7bd0955810", "uri": "../flows/98daf38a-7a79-46d3-9a37-2b7bd0955810.xml"}, "exchange direction": "OUTPUT", "other": {"anies": [{"name": "referenceToUnitGroupDataSet", "value": {"shortDescription": [{"value": "MJ", "lang": "de"}], "type": "unit group data set", "refObjectId": "93a60a57-a3c8-11da-a746-0800200c9a66", "uri": "../unitgroups/93a60a57-a3c8-11da-a746-0800200c9a66.xml"}}, {"value": "0", "module": "A1-A3"}, {"value": "0", "module": "A4"}, {"value": "0.0356541451751189", "module": "A5"}, {"value": "0", "module": "B2"}, {"value": "0", "module": "C1"}, {"value": "0", "module": "C2"}, {"value": "6.80328248134234", "module": "C3"}, {"value": "0", "module": "C4"}, {"value": "0", "module": "D"}]}, "resolvedFlowVersion": "38.00.000", "flowProperties": [], "typeOfFlow": "Other flow", "classification": {"classHierarchy": "Quantities / Environmental quantities / EPD EN 15804 / LCI indicators", "name": "GaBiCategories"}}]}, "LCIAResults": {"LCIAResult": [{"referenceToLCIAMethodDataSet": {"shortDescription": [{"value": "Globales Erwärmungspotenzial total (GWP-total)", "lang": "de"}, {"value": "Global Warming Potential total (GWP-total)", "lang": "en"}], "type": "LCIA method data set", "refObjectId": "6a37f984-a4b3-458a-a20a-64418c145fa2", "uri": "../lciamethods/6a37f984-a4b3-458a-a20a-64418c145fa2.xml"}, "other": {"anies": [{"name": "referenceToUnitGroupDataSet", "value": {"shortDescription": [{"value": "kg CO_(2)-Äq.", "lang": "de"}], "type": "unit group data set", "refObjectId": "1ebf3012-d0db-4de2-aefd-ef30cedb0be1", "uri": "../unitgroups/1ebf3012-d0db-4de2-aefd-ef30cedb0be1.xml"}}, {"value": "4.44243601229812", "module": "A1-A3"}, {"value": "0.228400412348228", "module": "A4"}, {"value": "0.386019219896422", "module": "A5"}, {"value": "0.0976656095666476", "module": "B2"}, {"value": "0.0325436184370899", "module": "C1"}, {"value": "0.00989516674184603", "module": "C2"}, {"value": "2.49714629492324", "module": "C3"}, {"value": "0", "module": "C4"}, {"value": "-0.849713580200998", "module": "D"}]}}, {"referenceToLCIAMethodDataSet": {"shortDescription": [{"value": "Globales Erwärmungspotenzial fossil (GWP-fossil)", "lang": "de"}, {"value": "Global Warming Potential fossil fuels (GWP-fossil)", "lang": "en"}], "type": "LCIA method data set", "refObjectId": "5f635281-343e-44fb-83df-1971b155e6b6", "uri": "../lciamethods/5f635281-343e-44fb-83df-1971b155e6b6.xml"}, "other": {"anies": [{"name": "referenceToUnitGroupDataSet", "value": {"shortDescription": [{"value": "kg CO_(2)-Äq.", "lang": "de"}], "type": "unit group data set", "refObjectId": "1ebf3012-d0db-4de2-aefd-ef30cedb0be1", "uri": "../unitgroups/1ebf3012-d0db-4de2-aefd-ef30cedb0be1.xml"}}, {"value": "5.57954971376987", "module": "A1-A3"}, {"value": "0.226089691322688", "module": "A4"}, {"value": "0.439529480982971", "module": "A5"}, {"value": "0.0929641241824758", "module": "B2"}, {"value": "0.0322596705162275", "module": "C1"}, {"value": "0.00978105989599964", "module": "C2"}, {"value": "1.05562001482379", "module": "C3"}, {"value": "0", "module": "C4"}, {"value": "-0.845776880744905", "module": "D"}]}}, {"referenceToLCIAMethodDataSet": {"shortDescription": [{"value": "Globales Erwärmungspotenzial biogen (GWP-biogenic)", "lang": "de"}, {"value": "Global Warming Potential biogenic (GWP-biogenic)", "lang": "en"}], "type": "LCIA method data set", "refObjectId": "2356e1ab-0185-4db5-86e5-16de51c7485c", "uri": "../lciamethods/2356e1ab-0185-4db5-86e5-16de51c7485c.xml"}, "other": {"anies": [{"name": "referenceToUnitGroupDataSet", "value": {"shortDescription": [{"value": "kg CO_(2)-Äq.", "lang": "de"}], "type": "unit group data set", "refObjectId": "1ebf3012-d0db-4de2-aefd-ef30cedb0be1", "uri": "../unitgroups/1ebf3012-d0db-4de2-aefd-ef30cedb0be1.xml"}}, {"value": "-1.67825972084906", "module": "A1-A3"}, {"value": "0.00047598501257963", "module": "A4"}, {"value": "-0.0811224323148709", "module": "A5"}, {"value": "0.00469994715908199", "module": "B2"}, {"value": "0.000280441493056765", "module": "C1"}, {"value": "2.23960223402636E-05", "module": "C2"}, {"value": "1.44151306862213", "module": "C3"}, {"value": "0", "module": "C4"}, {"value": "-0.00388138815219352", "module": "D"}]}}, {"referenceToLCIAMethodDataSet": {"shortDescription": [{"value": "Globales Erwärmungspotenzial luluc (GWP-luluc)", "lang": "de"}, {"value": "Global Warming Potential luluc (GWP-luluc)", "lang": "en"}], "type": "LCIA method data set", "refObjectId": "4331bbdb-978a-490d-8707-eeb047f01a55", "uri": "../lciamethods/4331bbdb-978a-490d-8707-eeb047f01a55.xml"}, "other": {"anies": [{"name": "referenceToUnitGroupDataSet", "value": {"shortDescription": [{"value": "kg CO_(2)-Äq.", "lang": "de"}], "type": "unit group data set", "refObjectId": "1ebf3012-d0db-4de2-aefd-ef30cedb0be1", "uri": "../unitgroups/1ebf3012-d0db-4de2-aefd-ef30cedb0be1.xml"}}, {"value": "0.541146019377316", "module": "A1-A3"}, {"value": "0.00183473601296027", "module": "A4"}, {"value": "0.0276121712283223", "module": "A5"}, {"value": "1.5382250897199E-06", "module": "B2"}, {"value": "3.50642780562094E-06", "module": "C1"}, {"value": "9.17108235061216E-05", "module": "C2"}, {"value": "1.3211477326086E-05", "module": "C3"}, {"value": "0", "module": "C4"}, {"value": "-5.53113038998742E-05", "module": "D"}]}}, {"referenceToLCIAMethodDataSet": {"shortDescription": [{"value": "Abbau Potential der stratosphärischen Ozonschicht (ODP)", "lang": "de"}, {"value": "Depletion potential of the stratospheric ozone layer (ODP)", "lang": "en"}], "type": "LCIA method data set", "refObjectId": "b5c629d6-def3-11e6-bf01-fe55135034f3", "uri": "../lciamethods/b5c629d6-def3-11e6-bf01-fe55135034f3.xml"}, "other": {"anies": [{"name": "referenceToUnitGroupDataSet", "value": {"shortDescription": [{"value": "kg CFC11-Äq.", "lang": "de"}], "type": "unit group data set", "refObjectId": "d9e957c9-7309-4474-bf3a-7777df6c4e5b", "uri": "../unitgroups/d9e957c9-7309-4474-bf3a-7777df6c4e5b.xml"}}, {"value": "1.4649498373512E-08", "module": "A1-A3"}, {"value": "2.7838389760381E-14", "module": "A4"}, {"value": "7.44960965802542E-10", "module": "A5"}, {"value": "8.11099503472155E-12", "module": "B2"}, {"value": "5.95266988800881E-13", "module": "C1"}, {"value": "1.28847568620027E-15", "module": "C2"}, {"value": "1.62060894820352E-13", "module": "C3"}, {"value": "0", "module": "C4"}, {"value": "-6.68604616648066E-12", "module": "D"}]}}, {"referenceToLCIAMethodDataSet": {"shortDescription": [{"value": "Versauerungspotenzial von Boden und Wasser (AP)", "lang": "de"}, {"value": "Acidification potential of land and water (AP)", "lang": "en"}], "type": "LCIA method data set", "refObjectId": "b5c611c6-def3-11e6-bf01-fe55135034f3", "uri": "../lciamethods/b5c611c6-def3-11e6-bf01-fe55135034f3.xml"}, "other": {"anies": [{"name": "referenceToUnitGroupDataSet", "value": {"shortDescription": [{"value": "mol H^(+)-Äq.", "lang": "de"}], "type": "unit group data set", "refObjectId": "42e089ac-92bf-4bf2-8ca1-5fc40d18f2ed", "uri": "../unitgroups/42e089ac-92bf-4bf2-8ca1-5fc40d18f2ed.xml"}}, {"value": "0.0373804860599307", "module": "A1-A3"}, {"value": "0.00170884764140887", "module": "A4"}, {"value": "0.00200238019320224", "module": "A5"}, {"value": "0.000294054388581696", "module": "B2"}, {"value": "6.89000731500695E-05", "module": "C1"}, {"value": "3.19522008424065E-05", "module": "C2"}, {"value": "0.000240875338765395", "module": "C3"}, {"value": "0", "module": "C4"}, {"value": "-0.00106137869581311", "module": "D"}]}}, {"referenceToLCIAMethodDataSet": {"shortDescription": [{"value": "Eutrophierungspotenzial Süßwasser (EP-freshwater)", "lang": "de"}, {"value": "Eutrophication potential aquatic freshwater (EP-freshwater)", "lang": "en"}], "type": "LCIA method data set", "refObjectId": "b53ec18f-7377-4ad3-86eb-cc3f4f276b2b", "uri": "../lciamethods/b53ec18f-7377-4ad3-86eb-cc3f4f276b2b.xml"}, "other": {"anies": [{"name": "referenceToUnitGroupDataSet", "value": {"shortDescription": [{"value": "kg P-Äq.", "lang": "de"}], "type": "unit group data set", "refObjectId": "0429039d-a61d-4590-ba67-aa4a20a810a1", "uri": "../unitgroups/0429039d-a61d-4590-ba67-aa4a20a810a1.xml"}}, {"value": "0.000694722723844154", "module": "A1-A3"}, {"value": "7.30993556419866E-07", "module": "A4"}, {"value": "3.53689142458377E-05", "module": "A5"}, {"value": "5.60741658871437E-06", "module": "B2"}, {"value": "1.20349557723587E-07", "module": "C1"}, {"value": "3.62043884504254E-08", "module": "C2"}, {"value": "6.91624798612707E-08", "module": "C3"}, {"value": "0", "module": "C4"}, {"value": "-1.37905294167488E-06", "module": "D"}]}}, {"referenceToLCIAMethodDataSet": {"shortDescription": [{"value": "Eutrophierungspotenzial Salzwasser (EP-marine)", "lang": "de"}, {"value": "Eutrophication potential aquatic marine (EP-marine)", "lang": "en"}], "type": "LCIA method data set", "refObjectId": "b5c619fa-def3-11e6-bf01-fe55135034f3", "uri": "../lciamethods/b5c619fa-def3-11e6-bf01-fe55135034f3.xml"}, "other": {"anies": [{"name": "referenceToUnitGroupDataSet", "value": {"shortDescription": [{"value": "kg N-Äq.", "lang": "de"}], "type": "unit group data set", "refObjectId": "d05bb823-ecdf-4686-8c40-bf1d9257859f", "uri": "../unitgroups/d05bb823-ecdf-4686-8c40-bf1d9257859f.xml"}}, {"value": "0.00700954483917275", "module": "A1-A3"}, {"value": "0.000540930392287295", "module": "A4"}, {"value": "0.000387752090935669", "module": "A5"}, {"value": "7.2297124390965E-05", "module": "B2"}, {"value": "1.648473098396E-05", "module": "C1"}, {"value": "1.44747826408015E-05", "module": "C2"}, {"value": "6.27979332393853E-05", "module": "C3"}, {"value": "0", "module": "C4"}, {"value": "-0.000309981666300081", "module": "D"}]}}, {"referenceToLCIAMethodDataSet": {"shortDescription": [{"value": "Eutrophierungspotenzial Land (EP-terrestrial)", "lang": "de"}, {"value": "Eutrophication potential terrestrial (EP-terrestrial)", "lang": "en"}], "type": "LCIA method data set", "refObjectId": "b5c614d2-def3-11e6-bf01-fe55135034f3", "uri": "../lciamethods/b5c614d2-def3-11e6-bf01-fe55135034f3.xml"}, "other": {"anies": [{"name": "referenceToUnitGroupDataSet", "value": {"shortDescription": [{"value": "mol N-Äq.", "lang": "de"}], "type": "unit group data set", "refObjectId": "71b4d617-0ec9-4d3f-b65e-e438940c2401", "uri": "../unitgroups/71b4d617-0ec9-4d3f-b65e-e438940c2401.xml"}}, {"value": "0.0945767956327264", "module": "A1-A3"}, {"value": "0.00600893615070022", "module": "A4"}, {"value": "0.00518356600982417", "module": "A5"}, {"value": "0.000558631167170453", "module": "B2"}, {"value": "0.000172247725539726", "module": "C1"}, {"value": "0.000162762655603172", "module": "C2"}, {"value": "0.00113683179457457", "module": "C3"}, {"value": "0", "module": "C4"}, {"value": "-0.00331838779259356", "module": "D"}]}}, {"referenceToLCIAMethodDataSet": {"shortDescription": [{"value": "Bildungspotential für troposphärisches Ozon (POCP)", "lang": "de"}, {"value": "Formation potential of tropospheric ozone photochemical oxidants (POCP)", "lang": "en"}], "type": "LCIA method data set", "refObjectId": "b5c610fe-def3-11e6-bf01-fe55135034f3", "uri": "../lciamethods/b5c610fe-def3-11e6-bf01-fe55135034f3.xml"}, "other": {"anies": [{"name": "referenceToUnitGroupDataSet", "value": {"shortDescription": [{"value": "kg NMVOC-Äq.", "lang": "de"}], "type": "unit group data set", "refObjectId": "d27c25f8-fbc1-44c6-b47b-4adbae4199c6", "uri": "../unitgroups/d27c25f8-fbc1-44c6-b47b-4adbae4199c6.xml"}}, {"value": "0.0209459987974104", "module": "A1-A3"}, {"value": "0.00129405447249965", "module": "A4"}, {"value": "0.00114174837310696", "module": "A5"}, {"value": "0.000294874250555615", "module": "B2"}, {"value": "4.39784262164529E-05", "module": "C1"}, {"value": "2.88906816208323E-05", "module": "C2"}, {"value": "0.000178700361280942", "module": "C3"}, {"value": "0", "module": "C4"}, {"value": "-0.000863412136555979", "module": "D"}]}}, {"referenceToLCIAMethodDataSet": {"shortDescription": [{"value": "Potenzial für den abiotischen Abbau nicht fossiler Ressourcen (ADPE)", "lang": "de"}, {"value": "Abiotic depletion potential for non fossil resources (ADPE)", "lang": "en"}], "type": "LCIA method data set", "refObjectId": "b2ad6494-c78d-11e6-9d9d-cec0c932ce01", "uri": "../lciamethods/b2ad6494-c78d-11e6-9d9d-cec0c932ce01.xml"}, "other": {"anies": [{"name": "referenceToUnitGroupDataSet", "value": {"shortDescription": [{"value": "kg Sb-Äq.", "lang": "de"}], "type": "unit group data set", "refObjectId": "54ccd2d9-a32a-4fc2-923d-f2c8c93e89d4", "uri": "../unitgroups/54ccd2d9-a32a-4fc2-923d-f2c8c93e89d4.xml"}}, {"value": "0.000144473163578374", "module": "A1-A3"}, {"value": "1.34049614506036E-08", "module": "A4"}, {"value": "7.34746123233253E-06", "module": "A5"}, {"value": "1.64854570208129E-08", "module": "B2"}, {"value": "4.98945007650019E-09", "module": "C1"}, {"value": "6.56537279787083E-10", "module": "C2"}, {"value": "1.57102659367781E-09", "module": "C3"}, {"value": "0", "module": "C4"}, {"value": "-6.1053397849829E-08", "module": "D"}]}}, {"referenceToLCIAMethodDataSet": {"shortDescription": [{"value": "Potenzial für den abiotischen Abbau fossiler Brennstoffe (ADPF)", "lang": "de"}, {"value": "Abiotic depletion potential for fossil resources (ADPF)", "lang": "en"}], "type": "LCIA method data set", "refObjectId": "b2ad6110-c78d-11e6-9d9d-cec0c932ce01", "uri": "../lciamethods/b2ad6110-c78d-11e6-9d9d-cec0c932ce01.xml"}, "other": {"anies": [{"name": "referenceToUnitGroupDataSet", "value": {"shortDescription": [{"value": "MJ", "lang": "de"}], "type": "unit group data set", "refObjectId": "93a60a57-a3c8-11da-a746-0800200c9a66", "uri": "../unitgroups/93a60a57-a3c8-11da-a746-0800200c9a66.xml"}}, {"value": "110.073416756971", "module": "A1-A3"}, {"value": "3.06390920073887", "module": "A4"}, {"value": "5.77709890164863", "module": "A5"}, {"value": "2.32540338417642", "module": "B2"}, {"value": "0.678887523500628", "module": "C1"}, {"value": "0.134895887655408", "module": "C2"}, {"value": "0.399754031413212", "module": "C3"}, {"value": "0", "module": "C4"}, {"value": "-15.6317323176514", "module": "D"}]}}, {"referenceToLCIAMethodDataSet": {"shortDescription": [{"value": "Wassernutzung (WDP)", "lang": "de"}, {"value": "Water use (WDP)", "lang": "en"}], "type": "LCIA method data set", "refObjectId": "b2ad66ce-c78d-11e6-9d9d-cec0c932ce01", "uri": "../lciamethods/b2ad66ce-c78d-11e6-9d9d-cec0c932ce01.xml"}, "other": {"anies": [{"name": "referenceToUnitGroupDataSet", "value": {"shortDescription": [{"value": "m^(3) Welt-Äq. entzogen", "lang": "de"}], "type": "unit group data set", "refObjectId": "6ae2df01-888e-46c8-b17d-49fa3869b476", "uri": "../unitgroups/6ae2df01-888e-46c8-b17d-49fa3869b476.xml"}}, {"value": "13.1080576734084", "module": "A1-A3"}, {"value": "0.00244354484376635", "module": "A4"}, {"value": "0.679560598387869", "module": "A5"}, {"value": "0.0159794102491602", "module": "B2"}, {"value": "0.00718907633720711", "module": "C1"}, {"value": "0.000119658644619948", "module": "C2"}, {"value": "0.213971386146131", "module": "C3"}, {"value": "0", "module": "C4"}, {"value": "-0.0810039609197269", "module": "D"}]}}, {"referenceToLCIAMethodDataSet": {"shortDescription": [{"value": "Auftreten von Krankheiten aufgrund von Feinstaubemissionen (PM)", "lang": "de"}, {"value": "Incidence of disease due to PM emissions (PM)", "lang": "en"}], "type": "LCIA method data set", "refObjectId": "b5c602c6-def3-11e6-bf01-fe55135034f3", "uri": "../lciamethods/b5c602c6-def3-11e6-bf01-fe55135034f3.xml"}, "other": {"anies": [{"name": "referenceToUnitGroupDataSet", "value": {"shortDescription": [{"value": "Krankheitsfälle", "lang": "de"}], "type": "unit group data set", "refObjectId": "3883559b-648f-4afc-8ba2-0bd24f3affa3", "uri": "../unitgroups/3883559b-648f-4afc-8ba2-0bd24f3affa3.xml"}}, {"value": "4.55645648736368E-07", "module": "A1-A3"}, {"value": "2.2559801769407E-08", "module": "A4"}, {"value": "2.44521626710382E-08", "module": "A5"}, {"value": "3.80559870411732E-09", "module": "B2"}, {"value": "5.79960438353899E-10", "module": "C1"}, {"value": "1.97183194817488E-10", "module": "C2"}, {"value": "2.28872741131972E-09", "module": "C3"}, {"value": "0", "module": "C4"}, {"value": "-9.00525200692411E-09", "module": "D"}]}}, {"referenceToLCIAMethodDataSet": {"shortDescription": [{"value": "Wirkung durch Exposition des Menschen mit U235 (IR)", "lang": "de"}, {"value": "Human exposure efficiency relative to U235 (IR)", "lang": "en"}], "type": "LCIA method data set", "refObjectId": "b5c632be-def3-11e6-bf01-fe55135034f3", "uri": "../lciamethods/b5c632be-def3-11e6-bf01-fe55135034f3.xml"}, "other": {"anies": [{"name": "referenceToUnitGroupDataSet", "value": {"shortDescription": [{"value": "kBq U235-Äq.", "lang": "de"}], "type": "unit group data set", "refObjectId": "456b05bf-1415-44a9-9993-02452f554c09", "uri": "../unitgroups/456b05bf-1415-44a9-9993-02452f554c09.xml"}}, {"value": "0.146948906629445", "module": "A1-A3"}, {"value": "0.000818067852848206", "module": "A4"}, {"value": "0.00772917091997396", "module": "A5"}, {"value": "0.0369355906244859", "module": "B2"}, {"value": "0.0179630403745954", "module": "C1"}, {"value": "3.77892314260569E-05", "module": "C2"}, {"value": "0.00358612521827843", "module": "C3"}, {"value": "0", "module": "C4"}, {"value": "-0.201512310278714", "module": "D"}]}}, {"referenceToLCIAMethodDataSet": {"shortDescription": [{"value": "Toxizitätsvergleichseinheit für Ökosysteme (ETP-fw)", "lang": "de"}, {"value": "Comparative toxic unit for ecosystems (ETP-fw)", "lang": "en"}], "type": "LCIA method data set", "refObjectId": "ee1082d1-b0f7-43ca-a1f0-21e2a4a74511", "uri": "../lciamethods/ee1082d1-b0f7-43ca-a1f0-21e2a4a74511.xml"}, "other": {"anies": [{"name": "referenceToUnitGroupDataSet", "value": {"shortDescription": [{"value": "CTUe", "lang": "de"}], "type": "unit group data set", "refObjectId": "aa959ded-f1eb-4efb-9c5c-2d60be36b3e6", "uri": "../unitgroups/aa959ded-f1eb-4efb-9c5c-2d60be36b3e6.xml"}}, {"value": "83.7135188279198", "module": "A1-A3"}, {"value": "2.19105233072535", "module": "A4"}, {"value": "4.37954499611679", "module": "A5"}, {"value": "0.520835653712767", "module": "B2"}, {"value": "0.188655083238538", "module": "C1"}, {"value": "0.0966278365353275", "module": "C2"}, {"value": "0.188945182209963", "module": "C3"}, {"value": "0", "module": "C4"}, {"value": "-2.18667361153118", "module": "D"}]}}, {"referenceToLCIAMethodDataSet": {"shortDescription": [{"value": "Toxizitätsvergleichseinheit für Menschen (krebserregend) (HTP-c)", "lang": "de"}, {"value": "Comparative toxic unit for humans (carcinogenic) (HTP-c)", "lang": "en"}], "type": "LCIA method data set", "refObjectId": "2299222a-bbd8-474f-9d4f-4dd1f18aea7c", "uri": "../lciamethods/2299222a-bbd8-474f-9d4f-4dd1f18aea7c.xml"}, "other": {"anies": [{"name": "referenceToUnitGroupDataSet", "value": {"shortDescription": [{"value": "CTUh", "lang": "de"}], "type": "unit group data set", "refObjectId": "d4c9523e-2d7e-49fd-8469-998f547d3a70", "uri": "../unitgroups/d4c9523e-2d7e-49fd-8469-998f547d3a70.xml"}}, {"value": "3.308090611008E-09", "module": "A1-A3"}, {"value": "4.3928638623844E-11", "module": "A4"}, {"value": "1.71397335713871E-10", "module": "A5"}, {"value": "3.65552029846391E-11", "module": "B2"}, {"value": "9.98921128570414E-12", "module": "C1"}, {"value": "1.96069674039779E-12", "module": "C2"}, {"value": "1.54871347393716E-11", "module": "C3"}, {"value": "0", "module": "C4"}, {"value": "-1.73274926010858E-10", "module": "D"}]}}, {"referenceToLCIAMethodDataSet": {"shortDescription": [{"value": "Toxizitätsvergleichseinheit für Menschen (nicht krebserregend) (HTP-nc)", "lang": "de"}, {"value": "Comparative toxic unit for humans (noncarcinogenic) (HTP-nc)", "lang": "en"}], "type": "LCIA method data set", "refObjectId": "3af763a5-b7a1-48c9-9cee-1f223481fcef", "uri": "../lciamethods/3af763a5-b7a1-48c9-9cee-1f223481fcef.xml"}, "other": {"anies": [{"name": "referenceToUnitGroupDataSet", "value": {"shortDescription": [{"value": "CTUh", "lang": "de"}], "type": "unit group data set", "refObjectId": "d4c9523e-2d7e-49fd-8469-998f547d3a70", "uri": "../unitgroups/d4c9523e-2d7e-49fd-8469-998f547d3a70.xml"}}, {"value": "1.90851121228551E-07", "module": "A1-A3"}, {"value": "1.89532141556477E-09", "module": "A4"}, {"value": "9.81975845319602E-09", "module": "A5"}, {"value": "3.04259945196637E-09", "module": "B2"}, {"value": "1.59236384350205E-10", "module": "C1"}, {"value": "8.72336890153357E-11", "module": "C2"}, {"value": "2.80805545243563E-10", "module": "C3"}, {"value": "0", "module": "C4"}, {"value": "-4.25446102051065E-09", "module": "D"}]}}, {"referenceToLCIAMethodDataSet": {"shortDescription": [{"value": "Bodenqualitätsindex (SQP)", "lang": "de"}, {"value": "Soil quality index (SQP)", "lang": "en"}], "type": "LCIA method data set", "refObjectId": "b2ad6890-c78d-11e6-9d9d-cec0c932ce01", "uri": "../lciamethods/b2ad6890-c78d-11e6-9d9d-cec0c932ce01.xml"}, "other": {"anies": [{"name": "referenceToUnitGroupDataSet", "value": {"shortDescription": [{"value": "SQP", "lang": "de"}], "type": "unit group data set", "refObjectId": "f130951c-e67f-4f7f-8dd4-665de3974e18", "uri": "../unitgroups/f130951c-e67f-4f7f-8dd4-665de3974e18.xml"}}, {"value": "511.603569210156", "module": "A1-A3"}, {"value": "1.12851341099162", "module": "A4"}, {"value": "26.0808171627447", "module": "A5"}, {"value": "0.0350532551272193", "module": "B2"}, {"value": "0.266424721171552", "module": "C1"}, {"value": "0.0563649329142801", "module": "C2"}, {"value": "0.12728807683593", "module": "C3"}, {"value": "0", "module": "C4"}, {"value": "-3.0017211004057", "module": "D"}]}}]}, "otherAttributes": {"{http://www.indata.network/EPD/2019}epd-version": "1.2"}, "version": "1.1", "locations": "../ILCDLocations.xml"}