{"processInformation": {"dataSetInformation": {"UUID": "7e67347c-c1c0-4e66-a982-5468f0ec585f", "name": {"baseName": [{"value": "PETtherm 50", "lang": "de"}, {"value": "PETtherm 50", "lang": "en"}], "functionalUnitFlowProperties": [{"lang": "de"}]}, "classificationInformation": {"classification": [{"class": [{"value": "Dämmstoffe", "level": 0, "classId": "2"}, {"value": "Polyethylen", "level": 1, "classId": "2.18"}, {"value": "Schaum", "level": 2, "classId": "2.18.01"}], "name": "OEKOBAU.DAT"}, {"class": [{"value": "02 Bauprodukte", "level": 0}, {"value": "Wärmedämmungsprodukte", "level": 1}, {"value": "Dämmstoffe aus Schaumkunststoffen", "level": 2}], "name": "IBUCategories"}]}, "generalComment": [{"value": "PETtherm 50 ist ein Polyethylenterephthalatschaum niedriger Dichte (PET) auf Basis von 100 % recycelten Kunststoffflaschen. Langfristige Stabilitt der Dmmeigenschaften und niedrige Wrmeleitfhigkeit sichern lebenslange Dmmleistung. Ausgezeichnete Wasserbestndigkeit und die geschlossenzellige Struktur des Materials sorgen auch nach vielen Jahren des Betriebs fr eine stabile Wrmeleitfhigkeit. Diese Eigenschaften verhindern zudem das Eindringen von Feuchtigkeit, Schimmel und Fulnis und bieten so einen langfristigen Korrosionsschutz und einen minimalen Wartungsaufwand. Darber hinaus kann das Material in geschwungene Formen thermogeformt, vorgefertigt oder vor Ort geschweit werden und ist fr fast jede Art von Veredelungsoptionen vielseitig einsetzbar. Seine thermoplastische Beschaffenheit ermglicht zudem eine vollstndige Recyclingfhigkeit des Materials nach der Nutzungsphase. \nPETtherm 50 basiert auf 100 % recyceltem PET und wird nach einem energie- und ressourcenoptimierten Produktionsprozess hergestellt: durch Wiederverwendung von Abfallmaterial und ohne Einsatz von ozonabbauenden HFKW- oder FCKW-Treibmitteln.", "lang": "de"}, {"value": "PETtherm 50 is a low-density polyethylene terephthalate foam (PET) based on 100% recycled plastic bottles. Long-term stability of the insulation properties and low thermal conductivity ensure lifelong insulation performance. Excellent water resistance and the closed-cell structure of the material ensure stable thermal conductivity even after many years of operation. These properties also prevent the penetration of moisture, mould and rot, thus offering long-term corrosion protection and minimum maintenance. In addition, the material can be thermoformed into curved shapes, prefabricated or welded on site, and is versatile for almost any type of finishing option. Its thermoplastic nature also means that the material can be fully recycled after the utilisation phase.\nPETtherm 50 is based on 100% recycled PET and is manufactured using an energy- and resource-optimised production process: by reusing waste material and without the use of ozone-depleting HFCs or CFC blowing agents.", "lang": "en"}]}, "quantitativeReference": {"referenceToReferenceFlow": [0]}, "time": {"referenceYear": 2024, "dataSetValidUntil": 2029, "other": {"anies": [{"name": "publicationDateOfEPD", "value": 1705017600000}]}}, "geography": {"locationOfOperationSupplyOrProduction": {"location": "RER"}}, "technology": {"technologyDescriptionAndIncludedProcesses": [{"value": "PETtherm 50 Schaumplatten werden auf der Basis von mechanisch recyceltem PET hergestellt. Diese Methode basiert auf der Wiederverwertung von PET-Abfällen nach der Trennung des Polymers von Verunreinigungen, um recycelte Flakes herzustellen. Es umfasst das Sortieren und Trennen der Abfälle, das Waschen zur Entfernung von Schmutz und Verunreinigungen sowie das weitere Mahlen, Zerkleinern und Sortieren durch die Zulieferer. Das recycelte Produkt entspricht den vorgegebenen Spezifikationen und wird in Form von Flakes und Granulat geliefert. Die Flakes werden durch Schmelzextrusion zu Granulat verarbeitet. Bei der Granulierung werden die Flocken vorgetrocknet, um eine hydrolytische Reaktion während des Extrusionsprozesses zu vermeiden. Die vorgetrockneten Flakes werden in einen Extruder eingespeist, wo das Material geschmolzen und homogenisiert wird. In einem Vakuumextraktionsbereich werden leichtflüchtige Verunreinigungen aus der Schmelze entfernt. Nach der abschließenden Filtration wird das Material durch Unterwasserschneiden granuliert, gefolgt von der Kristallisation des erhaltenen rPET-Granulats. Das so gewonnene recycelte PET-Granulat wird durch Schaumextrusion mittels eines halogenfreien überkritischen Fluids, das als physikalisches Treibmittel verwendet wird, zu Schaum weiterverarbeitet. Weitere Bestandteile des Schaums sind Additive zur Schaumnukleierung, Zellstabilisierung und Schmelzmodifizierung. Die patentierte Methode der rPET-Verarbeitung und -Modifikation während der Schmelzeverarbeitung ermöglicht es, den Hauptnachteil des mechanischen Recyclings - eine Verschlechterung der Produktqualität - zu umgehen und die Qualität trotz des thermischen Abbaus, der Photooxidation und der mechanischen Beanspruchung zu verbessern. Ein weiterer Bestandteil der Formulierung ist \"PET-Agglomerat\", das aus aufbereitetem PET-Schaum gewonnen wird. Die Hauptquelle für das Agglomerat ist der PET-Staub, der bei den seitlichen und oberflächlichen Fräsvorgängen im Anschluss an den Schaumextrusionsprozess (interner Kreislauf) entsteht. Eine weitere Quelle für Agglomerate ist PET-Schaum, der aus dem Abfallstrom anderer PET-Schaumprodukte entnommen wird. Alle zurückgewonnenen Schaumstoff-Abschnitte werden in einem ersten Schritt zerkleinert und verdichtet. Im zweiten Schritt werden die vorverdichteten Teile mit zurückgewonnenem PET-Staub gemischt und durch Scherkräfte teilweise aufgeschmolzen und durch eine Matrize zu einem Agglomerat geformt. Die extrudierten geschäumten PET-Platten mit homogener und geschlossenzelliger Struktur werden kalibriert, an den Kanten geschnitten und an der Oberfläche geschliffen, um das Endprodukt mit den erforderlichen Abmessungen und der gewünschten Ebenheit zu erhalten. \nTechnische Daten: \nWeitere technische Daten finden Sie im Produktdatenblatt, das auf der Website. Die akustischen Eigenschaften sind fr PETtherm 50 nicht relevant. \nDeklarierte Einheit: \nDas deklarierte Produkt ist PETtherm 50. Die deklarierte Einheit bezieht sich auf 1 m des Produkts. Die Verpackung ist mit 3,039 kg in der Berechnung ebenfalls enthalten. Die folgende Tabelle zeigt die Daten der deklarierten Einheit.", "lang": "de"}, {"value": "PETtherm 50 foam sheets are manufactured on the basis of mechanically recycled PET. This method is based on recycling PET waste after separating the polymer from impurities to produce recycled flakes. It involves sorting and separating the waste, washing to remove dirt and impurities and further grinding, shredding and sorting by the suppliers. The recycled product meets the given specifications and is supplied in the form of flakes and granulate. The flakes are processed into pellets by melt extrusion. During granulation, the flakes are pre-dried to avoid a hydrolytic reaction during the extrusion process. The pre-dried flakes are fed into an extruder, where the material is melted and homogenised. Volatile impurities are removed from the melt in a vacuum extraction area. After final filtration, the material is granulated by underwater cutting, followed by crystallisation of the resulting rPET pellets. The recycled PET pellets obtained in this way are further processed into foam by foam extrusion using a halogen-free supercritical fluid as a physical blowing agent. Other components of the foam are additives for foam nucleation, cell stabilisation and melt modification. The patented method of rPET processing and modification during melt processing makes it possible to avoid the main disadvantage of mechanical recycling - a deterioration in product quality - and to improve quality despite thermal degradation, photo-oxidation and mechanical stress. Another component of the formulation is ‘PET agglomerate’, which is obtained from recycled PET foam. The main source of agglomerate is the PET dust produced during the lateral and surface milling processes following the foam extrusion process (internal cycle). Another source of agglomerates is PET foam taken from the waste stream of other PET foam products. All recovered foam offcuts are shredded and compacted in a first step. In the second step, the pre-compacted parts are mixed with recovered PET dust and partially melted by shear forces and moulded into an agglomerate by a die. The extruded foamed PET sheets with a homogeneous and closed-cell structure are calibrated, cut at the edges and sanded on the surface to obtain the final product with the required dimensions and flatness. \nTechnical data: \nFurther technical data can be found in the product data sheet, which is available on the website. The acoustic properties are not relevant for PETtherm 50. \nDeclared unit: \nThe declared product is PETtherm 50. The declared unit refers to 1 m of the product. The packaging is also included in the calculation at 3.039 kg. The following table shows the data relating to the declared unit.", "lang": "en"}], "technologicalApplicability": [{"value": "PETtherm 50 bietet eine Lsung fr die (halb-) strukturelle Dmmung von Gebudehllen, Dchern, Bden und Innentrennwnden in Neubauten und bei der Renovierung lterer Gebude. \nDie bestimmungsgeme Verwendung gem ETA Nr. 21/0623 ist die Wrmedmmung von Wnden (einschlielich Kellerwnden), Decken, Bden, Dchern, Zwischensparren und Holzkonstruktionen. Die in der ETA festgelegten Anforderungen beruhen auf einer angenommenen Nutzungsdauer von 50 Jahren fr das Dmmstoffprodukt. Die Angaben zur Nutzungsdauer knnen nicht als Garantie des Herstellers ausgelegt werden, sondern sind lediglich als Hilfsmittel fr die Auswahl des richtigen Produkts im Hinblick auf die erwartete angemessene Nutzungsdauer der Konstruktion zu betrachten.", "lang": "de"}, {"value": "PETtherm 50 offers a solution for the (semi-)structural insulation of building shells, roofs, floors and interior partition walls in new buildings and in the renovation of older buildings.\nThe intended use according to ETA No. 21/0623 is the thermal insulation of walls (including basement walls), ceilings, floors, roofs, rafters, and timber constructions. The requirements specified in the ETA are based on an assumed service life of 50 years for the insulation product. The information on the service life cannot be interpreted as a guarantee by the manufacturer, but should only be regarded as an aid for selecting the right product with regard to the expected appropriate service life of the structure.", "lang": "en"}]}}, "modellingAndValidation": {"LCIMethodAndAllocation": {"typeOfDataSet": "EPD", "referenceToLCAMethodDetails": [{"shortDescription": [{"value": "Dämmstoffe aus Schaumkunststoffen.pdf", "lang": "de"}], "type": "source data set", "refObjectId": "e859d75e-16e7-488a-9f7c-cc335b880692"}], "other": {"anies": [{"name": "subType", "value": "specific dataset"}]}}, "dataSourcesTreatmentAndRepresentativeness": {"referenceToDataSource": [{"shortDescription": [{"value": "ecoinvent database (all versions)", "lang": "de"}], "type": "source data set", "refObjectId": "b497a91f-e14b-4b69-8f28-f50eb1576766"}, {"shortDescription": [{"value": "ecoinvent 3.9.1 database", "lang": "de"}], "type": "source data set", "refObjectId": "e2034c8f-9d74-46f2-8fce-1f0c5c5cebeb"}], "useAdviceForDataSet": [{"value": "Gültigkeitsbereich: \nDieses Dokument gilt fr PETtherm 50. Fr die Erstellung der kobilanz wurden spezifische Daten aus dem Produktionswerk in Belgien erhoben, die dem Jahresdurchschnitt entsprechen und auf Daten aus dem Jahr 2022 basieren (siehe Zuordnung 3.8). Der Erklrungsinhaber haftet fr die Informationen und Nachweise, auf denen sie basiert; die IBU bernimmt keine Haftung fr Herstellerinformationen, Lebenszyklusbewertungsdaten und Nachweise. \nSystemgrenze: \nTyp der EPD: von der Wiege bis zum Werkstor mit Optionen, Modulen C1-C4 und Modul D. Die folgenden Informationsmodule werden in dieser Studie als Systemgrenzen definiert: \n\nA1–A5 Produktentwicklung: \nA1 – Produktion von Rohstoffen \nA2 – Transport zum Hersteller \nA3 – Produktion \nA4 – Transport vom Werkstor zur Baustelle \nA5 – Montage der Produkte im Gebude \n\nEnde der Lebensdauer (C1–C4): \nC1 – Rckbau/Abbruch, \nC2 – Transport, \nC3 – Abfallbehandlung, \nC4 – Entsorgung. \n\nWiederverwendungs-, Verwertungs- und Recyclingpotenzial (D) \n\nUm die Indikatoren und Umweltauswirkungen der deklarierten Einheit genau zu erfassen, werden insgesamt 8 Informationsmodule bercksichtigt. Die Informationsmodule A1 bis A3 beschreiben die Bereitstellung von Materialien, den Transport zum Produktionsstandort sowie die Produktionsprozesse des Produktes selbst.", "lang": "de"}, {"value": "Scope: \nThis document applies to PETtherm 50. Specific data from the production plant in Belgium was collected for the preparation of the Life Cycle Assessment, which corresponds to the annual average and is based on data from 2022 (see Allocation 3.8). The owner of the Declaration shall be liable for the information and proof on which it is based: IBU shall not be liable with respect to manufacturer information, Life Cycle Assessment data, or proof. \nSystem boundary: \nType of EPD: from the cradle to the factory gate with options, Modules C1-C4 and Module D. The following information modules are defined as system boundaries in this study: \n\nA1-A5 Product development: \nA1 - Production of raw materials\nA2 - Transport to the manufacturer\nA3 - Production \nA4 - Transport from the factory gate to the construction site\nA5 - Assembly of the products in the building \n\nEnd of service life (C1-C4): \nC1 - Dismantling/demolition\nC2 - Transport \nC3 - Waste treatment\nC4 - Disposal \n\nReuse, recovery and recycling potential (D) \n\nIn order to accurately record the indicators and environmental impacts of the declared unit, a total of 8 information modules are taken into account. Information modules A1 to A3 describe the provision of materials, the transport to the production site, and the production processes of the product itself.", "lang": "en"}], "other": {"anies": [{"name": "referenceToOriginalEPD", "value": {"shortDescription": {"value": "PETtherm 50.pdf", "defaultValue": "PETtherm 50.pdf", "lstrings": [{"lang": "de", "value": "PETtherm 50.pdf"}]}, "type": "source data set", "uuid": {"uuid": "c134854d-390e-44ae-98a1-6ac969b957aa"}, "refObjectId": "c134854d-390e-44ae-98a1-6ac969b957aa", "resourceURLs": ["https://oekobaudat.de/OEKOBAU.DAT/resource/sources/c134854d-390e-44ae-98a1-6ac969b957aa/PETtherm_50_20737.pdf?version=00.01.000"]}}]}}, "validation": {"review": [{"referenceToNameOfReviewerAndInstitution": [{"shortDescription": [{"value": "Institut Bauen und Umwelt e. V.", "lang": "de"}], "type": "contact data set", "refObjectId": "d111dbec-b024-4be5-86c5-752d6eb2cf95", "uri": "../contacts/d111dbec-b024-4be5-86c5-752d6eb2cf95.xml"}], "type": "Accredited third party review"}]}, "complianceDeclarations": {"compliance": [{"referenceToComplianceSystem": {"shortDescription": [{"value": "DIN EN 15804+A2", "lang": "de"}], "type": "source data set", "refObjectId": "c0016b33-8cf7-415c-ac6e-deba0d21440d", "uri": "../sources/c0016b33-8cf7-415c-ac6e-deba0d21440d.xml"}}, {"referenceToComplianceSystem": {"shortDescription": [{"value": "ISO 14025", "lang": "de"}], "type": "source data set", "refObjectId": "4f2eb655-6e44-4874-a95a-e28f5442cd4d", "uri": "../sources/4f2eb655-6e44-4874-a95a-e28f5442cd4d.xml"}}]}}, "administrativeInformation": {"commissionerAndGoal": {"referenceToCommissioner": [{"shortDescription": [{"value": "Pflüger TOB GmbH", "lang": "de"}], "type": "contact data set", "refObjectId": "c1174014-222e-4fa2-90c0-2764dea55937", "uri": "../contacts/c1174014-222e-4fa2-90c0-2764dea55937.xml"}]}, "dataGenerator": {"referenceToPersonOrEntityGeneratingTheDataSet": [{"shortDescription": [{"value": "FIT-Umwelttechnik GmbH", "lang": "de"}], "type": "contact data set", "refObjectId": "702c9be1-2efc-4216-a011-35e36d30f038", "uri": "../contacts/702c9be1-2efc-4216-a011-35e36d30f038.xml"}]}, "dataEntryBy": {"timeStamp": 1705017600000, "referenceToDataSetFormat": [{"shortDescription": [{"value": "ILCD Format", "lang": "de"}], "type": "source data set", "refObjectId": "a97a0155-0234-4b87-b4ce-a45da52f2a40", "uri": "../sources/a97a0155-0234-4b87-b4ce-a45da52f2a40.xml"}, {"shortDescription": [{"value": "EPD-Datenformaterweiterungen v1.2", "lang": "de"}, {"value": "EPD Data Format Extensions v1.2", "lang": "en"}], "type": "source data set", "refObjectId": "a29449fd-aa2f-4de8-b5d7-4b06b43c6fde", "uri": "../sources/a29449fd-aa2f-4de8-b5d7-4b06b43c6fde.xml"}]}, "publicationAndOwnership": {"dataSetVersion": "00.04.000", "referenceToRegistrationAuthority": {"shortDescription": [{"value": "Institut Bauen und Umwelt e. V.", "lang": "de"}], "type": "contact data set", "refObjectId": "d111dbec-b024-4be5-86c5-752d6eb2cf95", "uri": "../contacts/d111dbec-b024-4be5-86c5-752d6eb2cf95.xml"}, "registrationNumber": "EPD-PFL-20240402-IBA1-DE", "referenceToOwnershipOfDataSet": {"shortDescription": [{"value": "Pflüger TOB GmbH", "lang": "de"}], "type": "contact data set", "refObjectId": "c1174014-222e-4fa2-90c0-2764dea55937", "uri": "../contacts/c1174014-222e-4fa2-90c0-2764dea55937.xml"}, "copyright": true, "licenseType": "Free of charge for all users and uses", "accessRestrictions": [{"value": "None", "lang": "en"}], "other": {"anies": [{"name": "referenceToPublisher", "value": {"shortDescription": [{"value": "Institut Bauen und Umwelt e. V.", "lang": "de"}], "type": "contact data set", "refObjectId": "d111dbec-b024-4be5-86c5-752d6eb2cf95", "uri": "../contacts/d111dbec-b024-4be5-86c5-752d6eb2cf95.xml"}}]}}}, "exchanges": {"exchange": [{"dataSetInternalID": 0, "referenceToFlowDataSet": {"shortDescription": [{"value": "PETtherm 50 (PETtherm 50)", "lang": "de"}], "type": "flow data set", "refObjectId": "c7715d80-c44c-fe49-c4ac-ea2529dd2c3c", "uri": "../flows/c7715d80-c44c-fe49-c4ac-ea2529dd2c3c.xml"}, "meanAmount": 1.0, "referencesToDataSource": {}, "referenceFlow": true, "resolvedFlowVersion": "00.04.000", "resultingflowAmount": 1.0, "flowProperties": [{"name": [{"lang": "en", "value": "Volume"}, {"lang": "de", "value": "Volumen"}], "uuid": "93a60a56-a3c8-22da-a746-0800200c9a66", "referenceFlowProperty": true, "meanValue": 1.0, "referenceUnit": "m3", "unitGroupUUID": "cd950537-0a98-4044-9ba7-9f9a68d0a504"}], "materialProperties": [{"name": "gross density", "value": "50.0", "unit": "kg/m^3", "unitDescription": "kilograms per cubic metre"}], "typeOfFlow": "Product flow", "classification": {"classHierarchy": "Dämmstoffe / Polyethylen / Schaum", "name": "OEKOBAU.DAT"}}, {"dataSetInternalID": 1, "referenceToFlowDataSet": {"shortDescription": [{"value": "Erneuerbare Primärenergie als Energieträger (PERE)", "lang": "de"}, {"value": "Renewable primary energy as energy carrier (PERE)", "lang": "en"}], "type": "flow data set", "refObjectId": "20f32be5-0398-4288-9b6d-accddd195317", "uri": "../flows/20f32be5-0398-4288-9b6d-accddd195317.xml"}, "exchange direction": "INPUT", "other": {"anies": [{"name": "referenceToUnitGroupDataSet", "value": {"shortDescription": [{"value": "MJ", "lang": "de"}], "type": "unit group data set", "refObjectId": "93a60a57-a3c8-11da-a746-0800200c9a66", "uri": "../unitgroups/93a60a57-a3c8-11da-a746-0800200c9a66.xml"}}, {"value": "375.47", "module": "A1-A3"}, {"value": "1.87", "module": "A4"}, {"value": "-3.85", "module": "A5"}, {"value": "0.676", "module": "C1"}, {"value": "0.176", "module": "C2"}, {"value": "18.9", "module": "C3"}, {"value": "0.245", "module": "C4"}, {"value": "-58.6", "module": "D"}]}, "resolvedFlowVersion": "38.00.000", "flowProperties": [], "typeOfFlow": "Other flow", "classification": {"classHierarchy": "Quantities", "name": "GaBiCategories"}}, {"dataSetInternalID": 2, "referenceToFlowDataSet": {"shortDescription": [{"value": "Erneuerbare Primärenergie zur stofflichen Nutzung (PERM)", "lang": "de"}, {"value": "Renewable primary energy resources as material utilization (PERM)", "lang": "en"}], "type": "flow data set", "refObjectId": "fb3ec0de-548d-4508-aea5-00b73bf6f702", "uri": "../flows/fb3ec0de-548d-4508-aea5-00b73bf6f702.xml"}, "exchange direction": "INPUT", "other": {"anies": [{"name": "referenceToUnitGroupDataSet", "value": {"shortDescription": [{"value": "MJ", "lang": "de"}], "type": "unit group data set", "refObjectId": "93a60a57-a3c8-11da-a746-0800200c9a66", "uri": "../unitgroups/93a60a57-a3c8-11da-a746-0800200c9a66.xml"}}, {"value": "7.6429046048634", "module": "A1-A3"}, {"value": "0", "module": "A4"}, {"value": "0", "module": "A5"}, {"value": "0", "module": "C1"}, {"value": "0", "module": "C2"}, {"value": "0", "module": "C3"}, {"value": "0", "module": "C4"}, {"value": "0", "module": "D"}]}, "resolvedFlowVersion": "38.00.000", "flowProperties": [], "typeOfFlow": "Other flow", "classification": {"classHierarchy": "Quantities", "name": "GaBiCategories"}}, {"dataSetInternalID": 3, "referenceToFlowDataSet": {"shortDescription": [{"value": "Total erneuerbare Primärenergie (PERT)", "lang": "de"}, {"value": "Total use of renewable primary energy resources (PERT)", "lang": "en"}], "type": "flow data set", "refObjectId": "53f97275-fa8a-4cdd-9024-65936002acd0", "uri": "../flows/53f97275-fa8a-4cdd-9024-65936002acd0.xml"}, "exchange direction": "INPUT", "other": {"anies": [{"name": "referenceToUnitGroupDataSet", "value": {"shortDescription": [{"value": "MJ", "lang": "de"}], "type": "unit group data set", "refObjectId": "93a60a57-a3c8-11da-a746-0800200c9a66", "uri": "../unitgroups/93a60a57-a3c8-11da-a746-0800200c9a66.xml"}}, {"value": "375.47", "module": "A1-A3"}, {"value": "1.87", "module": "A4"}, {"value": "-3.85", "module": "A5"}, {"value": "0.676", "module": "C1"}, {"value": "0.176", "module": "C2"}, {"value": "18.9", "module": "C3"}, {"value": "0.245", "module": "C4"}, {"value": "-58.6", "module": "D"}]}, "resolvedFlowVersion": "38.00.000", "flowProperties": [], "typeOfFlow": "Other flow", "classification": {"classHierarchy": "Quantities / Environmental quantities / EPD EN 15804 / LCI indicators", "name": "GaBiCategories"}}, {"dataSetInternalID": 4, "referenceToFlowDataSet": {"shortDescription": [{"value": "Nicht-erneuerbare Primärenergie als Energieträger (PENRE)", "lang": "de"}, {"value": "Non renewable primary energy as energy carrier (PENRE)", "lang": "en"}], "type": "flow data set", "refObjectId": "ac857178-2b45-46ec-892a-a9a4332f0372", "uri": "../flows/ac857178-2b45-46ec-892a-a9a4332f0372.xml"}, "exchange direction": "INPUT", "other": {"anies": [{"name": "referenceToUnitGroupDataSet", "value": {"shortDescription": [{"value": "MJ", "lang": "de"}], "type": "unit group data set", "refObjectId": "93a60a57-a3c8-11da-a746-0800200c9a66", "uri": "../unitgroups/93a60a57-a3c8-11da-a746-0800200c9a66.xml"}}, {"value": "1028.9", "module": "A1-A3"}, {"value": "26.4", "module": "A4"}, {"value": "-53.8", "module": "A5"}, {"value": "1.13", "module": "C1"}, {"value": "2.5", "module": "C2"}, {"value": "33.7", "module": "C3"}, {"value": "0.964", "module": "C4"}, {"value": "-473", "module": "D"}]}, "resolvedFlowVersion": "38.00.000", "flowProperties": [], "typeOfFlow": "Other flow", "classification": {"classHierarchy": "Quantities", "name": "GaBiCategories"}}, {"dataSetInternalID": 5, "referenceToFlowDataSet": {"shortDescription": [{"value": "Nicht-erneuerbare Primärenergie zur stofflichen Nutzung (PENRM)", "lang": "de"}, {"value": "Non renewable primary energy as material utilization (PENRM)", "lang": "en"}], "type": "flow data set", "refObjectId": "1421caa0-679d-4bf4-b282-0eb850ccae27", "uri": "../flows/1421caa0-679d-4bf4-b282-0eb850ccae27.xml"}, "exchange direction": "INPUT", "other": {"anies": [{"name": "referenceToUnitGroupDataSet", "value": {"shortDescription": [{"value": "MJ", "lang": "de"}], "type": "unit group data set", "refObjectId": "93a60a57-a3c8-11da-a746-0800200c9a66", "uri": "../unitgroups/93a60a57-a3c8-11da-a746-0800200c9a66.xml"}}, {"value": "4.395", "module": "A1-A3"}, {"value": "0", "module": "A4"}, {"value": "0", "module": "A5"}, {"value": "0", "module": "C1"}, {"value": "0", "module": "C2"}, {"value": "0", "module": "C3"}, {"value": "0", "module": "C4"}, {"value": "0", "module": "D"}]}, "resolvedFlowVersion": "38.00.000", "flowProperties": [], "typeOfFlow": "Other flow", "classification": {"classHierarchy": "Quantities", "name": "GaBiCategories"}}, {"dataSetInternalID": 6, "referenceToFlowDataSet": {"shortDescription": [{"value": "Total nicht erneuerbare Primärenergie (PENRT)", "lang": "de"}, {"value": "Total use of non renewable primary energy resources (PENRT)", "lang": "en"}], "type": "flow data set", "refObjectId": "06159210-646b-4c8d-8583-da9b3b95a6c1", "uri": "../flows/06159210-646b-4c8d-8583-da9b3b95a6c1.xml"}, "exchange direction": "INPUT", "other": {"anies": [{"name": "referenceToUnitGroupDataSet", "value": {"shortDescription": [{"value": "MJ", "lang": "de"}], "type": "unit group data set", "refObjectId": "93a60a57-a3c8-11da-a746-0800200c9a66", "uri": "../unitgroups/93a60a57-a3c8-11da-a746-0800200c9a66.xml"}}, {"value": "1028.9", "module": "A1-A3"}, {"value": "26.4", "module": "A4"}, {"value": "-53.8", "module": "A5"}, {"value": "1.13", "module": "C1"}, {"value": "2.5", "module": "C2"}, {"value": "33.7", "module": "C3"}, {"value": "0.964", "module": "C4"}, {"value": "-473", "module": "D"}]}, "resolvedFlowVersion": "38.00.000", "flowProperties": [], "typeOfFlow": "Other flow", "classification": {"classHierarchy": "Quantities / Environmental quantities / EPD EN 15804 / LCI indicators", "name": "GaBiCategories"}}, {"dataSetInternalID": 7, "referenceToFlowDataSet": {"shortDescription": [{"value": "Einsatz von Sekundärstoffen (SM)", "lang": "de"}, {"value": "Use of secondary material (SM)", "lang": "en"}], "type": "flow data set", "refObjectId": "c6a1f35f-2d09-4f54-8dfb-97e502e1ce92", "uri": "../flows/c6a1f35f-2d09-4f54-8dfb-97e502e1ce92.xml"}, "exchange direction": "INPUT", "other": {"anies": [{"name": "referenceToUnitGroupDataSet", "value": {"shortDescription": [{"value": "kg", "lang": "de"}], "type": "unit group data set", "refObjectId": "ad38d542-3fe9-439d-9b95-2f5f7752acaf", "uri": "../unitgroups/ad38d542-3fe9-439d-9b95-2f5f7752acaf.xml"}}, {"value": "23.067", "module": "A1-A3"}, {"value": "0", "module": "A4"}, {"value": "0", "module": "A5"}, {"value": "0", "module": "C1"}, {"value": "0", "module": "C2"}, {"value": "0", "module": "C3"}, {"value": "0", "module": "C4"}, {"value": "0", "module": "D"}]}, "resolvedFlowVersion": "38.00.000", "flowProperties": [], "typeOfFlow": "Other flow", "classification": {"classHierarchy": "Quantities / Environmental quantities / EPD EN 15804 / LCI indicators", "name": "GaBiCategories"}}, {"dataSetInternalID": 8, "referenceToFlowDataSet": {"shortDescription": [{"value": "Erneuerbare Sekundärbrennstoffe (RSF)", "lang": "de"}, {"value": "Use of renewable secondary fuels (RSF)", "lang": "en"}], "type": "flow data set", "refObjectId": "64333088-a55f-4aa2-9a31-c10b07816787", "uri": "../flows/64333088-a55f-4aa2-9a31-c10b07816787.xml"}, "exchange direction": "INPUT", "other": {"anies": [{"name": "referenceToUnitGroupDataSet", "value": {"shortDescription": [{"value": "MJ", "lang": "de"}], "type": "unit group data set", "refObjectId": "93a60a57-a3c8-11da-a746-0800200c9a66", "uri": "../unitgroups/93a60a57-a3c8-11da-a746-0800200c9a66.xml"}}, {"value": "0", "module": "A1-A3"}, {"value": "0", "module": "A4"}, {"value": "0", "module": "A5"}, {"value": "0", "module": "C1"}, {"value": "0", "module": "C2"}, {"value": "0", "module": "C3"}, {"value": "0", "module": "C4"}, {"value": "0", "module": "D"}]}, "resolvedFlowVersion": "38.00.000", "flowProperties": [], "typeOfFlow": "Other flow", "classification": {"classHierarchy": "Quantities / Environmental quantities / EPD EN 15804 / LCI indicators", "name": "GaBiCategories"}}, {"dataSetInternalID": 9, "referenceToFlowDataSet": {"shortDescription": [{"value": "Nicht erneuerbare Sekundärbrennstoffe (NRSF)", "lang": "de"}, {"value": "Use of non renewable secondary fuels (NRSF)", "lang": "en"}], "type": "flow data set", "refObjectId": "89def144-d39a-4287-b86f-efde453ddcb2", "uri": "../flows/89def144-d39a-4287-b86f-efde453ddcb2.xml"}, "exchange direction": "INPUT", "other": {"anies": [{"name": "referenceToUnitGroupDataSet", "value": {"shortDescription": [{"value": "MJ", "lang": "de"}], "type": "unit group data set", "refObjectId": "93a60a57-a3c8-11da-a746-0800200c9a66", "uri": "../unitgroups/93a60a57-a3c8-11da-a746-0800200c9a66.xml"}}, {"value": "0", "module": "A1-A3"}, {"value": "0", "module": "A4"}, {"value": "0", "module": "A5"}, {"value": "0", "module": "C1"}, {"value": "0", "module": "C2"}, {"value": "0", "module": "C3"}, {"value": "0", "module": "C4"}, {"value": "0", "module": "D"}]}, "resolvedFlowVersion": "38.00.000", "flowProperties": [], "typeOfFlow": "Other flow", "classification": {"classHierarchy": "Quantities / Environmental quantities / EPD EN 15804 / LCI indicators", "name": "GaBiCategories"}}, {"dataSetInternalID": 10, "referenceToFlowDataSet": {"shortDescription": [{"value": "Einsatz von Süßwasserressourcen (FW)", "lang": "de"}, {"value": "Use of net fresh water (FW)", "lang": "en"}], "type": "flow data set", "refObjectId": "3cf952c8-f3a4-461d-8c96-96456ca62246", "uri": "../flows/3cf952c8-f3a4-461d-8c96-96456ca62246.xml"}, "exchange direction": "INPUT", "other": {"anies": [{"name": "referenceToUnitGroupDataSet", "value": {"shortDescription": [{"value": "m^3", "lang": "de"}], "type": "unit group data set", "refObjectId": "cd950537-0a98-4044-9ba7-9f9a68d0a504", "uri": "../unitgroups/cd950537-0a98-4044-9ba7-9f9a68d0a504.xml"}}, {"value": "0.31152", "module": "A1-A3"}, {"value": "0.00206", "module": "A4"}, {"value": "0.0128", "module": "A5"}, {"value": "0.000546", "module": "C1"}, {"value": "0.000194", "module": "C2"}, {"value": "0.0158", "module": "C3"}, {"value": "0.0125", "module": "C4"}, {"value": "-0.229", "module": "D"}]}, "resolvedFlowVersion": "38.00.000", "flowProperties": [], "typeOfFlow": "Other flow", "classification": {"classHierarchy": "Quantities / Environmental quantities / EPD EN 15804 / LCI indicators", "name": "GaBiCategories"}}, {"dataSetInternalID": 11, "referenceToFlowDataSet": {"shortDescription": [{"value": "Gefährlicher Abfall zur Deponie (HWD)", "lang": "de"}, {"value": "Hazardous waste disposed (HWD)", "lang": "en"}], "type": "flow data set", "refObjectId": "430f9e0f-59b2-46a0-8e0d-55e0e84948fc", "uri": "../flows/430f9e0f-59b2-46a0-8e0d-55e0e84948fc.xml"}, "exchange direction": "OUTPUT", "other": {"anies": [{"name": "referenceToUnitGroupDataSet", "value": {"shortDescription": [{"value": "kg", "lang": "de"}], "type": "unit group data set", "refObjectId": "ad38d542-3fe9-439d-9b95-2f5f7752acaf", "uri": "../unitgroups/ad38d542-3fe9-439d-9b95-2f5f7752acaf.xml"}}, {"value": "1.0080772E-06", "module": "A1-A3"}, {"value": "9.78E-11", "module": "A4"}, {"value": "-6.12E-09", "module": "A5"}, {"value": "-8.86E-11", "module": "C1"}, {"value": "9.24E-12", "module": "C2"}, {"value": "-2.44E-09", "module": "C3"}, {"value": "2.21E-11", "module": "C4"}, {"value": "-1.75E-09", "module": "D"}]}, "resolvedFlowVersion": "38.00.000", "flowProperties": [], "typeOfFlow": "Other flow", "classification": {"classHierarchy": "Quantities / Environmental quantities / EPD EN 15804 / LCI indicators", "name": "GaBiCategories"}}, {"dataSetInternalID": 12, "referenceToFlowDataSet": {"shortDescription": [{"value": "Entsorgter nicht gefährlicher Abfall (NHWD)", "lang": "de"}, {"value": "Non hazardous waste disposed (NHWD)", "lang": "en"}], "type": "flow data set", "refObjectId": "b29ef66b-e286-4afa-949f-62f1a7b4d7fa", "uri": "../flows/b29ef66b-e286-4afa-949f-62f1a7b4d7fa.xml"}, "exchange direction": "OUTPUT", "other": {"anies": [{"name": "referenceToUnitGroupDataSet", "value": {"shortDescription": [{"value": "kg", "lang": "de"}], "type": "unit group data set", "refObjectId": "ad38d542-3fe9-439d-9b95-2f5f7752acaf", "uri": "../unitgroups/ad38d542-3fe9-439d-9b95-2f5f7752acaf.xml"}}, {"value": "0.25081", "module": "A1-A3"}, {"value": "0.00381", "module": "A4"}, {"value": "0.104", "module": "A5"}, {"value": "0.000829", "module": "C1"}, {"value": "0.00036", "module": "C2"}, {"value": "0.0235", "module": "C3"}, {"value": "0.0282", "module": "C4"}, {"value": "-0.0164", "module": "D"}]}, "resolvedFlowVersion": "38.00.000", "flowProperties": [], "typeOfFlow": "Other flow", "classification": {"classHierarchy": "Quantities / Environmental quantities / EPD EN 15804 / LCI indicators", "name": "GaBiCategories"}}, {"dataSetInternalID": 13, "referenceToFlowDataSet": {"shortDescription": [{"value": "Entsorgter radioaktiver Abfall (RWD)", "lang": "de"}, {"value": "Radioactive waste disposed (RWD)", "lang": "en"}], "type": "flow data set", "refObjectId": "3449546e-52ad-4b39-b809-9fb77cea8ff6", "uri": "../flows/3449546e-52ad-4b39-b809-9fb77cea8ff6.xml"}, "exchange direction": "OUTPUT", "other": {"anies": [{"name": "referenceToUnitGroupDataSet", "value": {"shortDescription": [{"value": "kg", "lang": "de"}], "type": "unit group data set", "refObjectId": "ad38d542-3fe9-439d-9b95-2f5f7752acaf", "uri": "../unitgroups/ad38d542-3fe9-439d-9b95-2f5f7752acaf.xml"}}, {"value": "0.093947", "module": "A1-A3"}, {"value": "3.42E-05", "module": "A4"}, {"value": "-0.00472", "module": "A5"}, {"value": "0.00018", "module": "C1"}, {"value": "3.23E-06", "module": "C2"}, {"value": "0.00499", "module": "C3"}, {"value": "5.81E-05", "module": "C4"}, {"value": "-0.00257", "module": "D"}]}, "resolvedFlowVersion": "38.00.000", "flowProperties": [], "typeOfFlow": "Other flow", "classification": {"classHierarchy": "Quantities / Environmental quantities / EPD EN 15804 / LCI indicators", "name": "GaBiCategories"}}, {"dataSetInternalID": 14, "referenceToFlowDataSet": {"shortDescription": [{"value": "Komponenten für die Wiederverwendung (CRU)", "lang": "de"}, {"value": "Components for re-use (CRU)", "lang": "en"}], "type": "flow data set", "refObjectId": "a2b32f97-3fc7-4af2-b209-525bc6426f33", "uri": "../flows/a2b32f97-3fc7-4af2-b209-525bc6426f33.xml"}, "exchange direction": "OUTPUT", "other": {"anies": [{"name": "referenceToUnitGroupDataSet", "value": {"shortDescription": [{"value": "kg", "lang": "de"}], "type": "unit group data set", "refObjectId": "ad38d542-3fe9-439d-9b95-2f5f7752acaf", "uri": "../unitgroups/ad38d542-3fe9-439d-9b95-2f5f7752acaf.xml"}}, {"value": "0", "module": "A1-A3"}, {"value": "0", "module": "A4"}, {"value": "0", "module": "A5"}, {"value": "0", "module": "C1"}, {"value": "0", "module": "C2"}, {"value": "0", "module": "C3"}, {"value": "0", "module": "C4"}, {"value": "0", "module": "D"}]}, "resolvedFlowVersion": "38.00.000", "flowProperties": [], "typeOfFlow": "Other flow", "classification": {"classHierarchy": "Quantities / Environmental quantities / EPD EN 15804 / LCI indicators", "name": "GaBiCategories"}}, {"dataSetInternalID": 15, "referenceToFlowDataSet": {"shortDescription": [{"value": "Stoffe zum Recycling (MFR)", "lang": "de"}, {"value": "Materials for recycling (MFR)", "lang": "en"}], "type": "flow data set", "refObjectId": "d7fe48a5-4103-49c8-9aae-b0b5dfdbd6ae", "uri": "../flows/d7fe48a5-4103-49c8-9aae-b0b5dfdbd6ae.xml"}, "exchange direction": "OUTPUT", "other": {"anies": [{"name": "referenceToUnitGroupDataSet", "value": {"shortDescription": [{"value": "kg", "lang": "de"}], "type": "unit group data set", "refObjectId": "ad38d542-3fe9-439d-9b95-2f5f7752acaf", "uri": "../unitgroups/ad38d542-3fe9-439d-9b95-2f5f7752acaf.xml"}}, {"value": "0", "module": "A1-A3"}, {"value": "0", "module": "A4"}, {"value": "0", "module": "A5"}, {"value": "0", "module": "C1"}, {"value": "0", "module": "C2"}, {"value": "0", "module": "C3"}, {"value": "0", "module": "C4"}, {"value": "0", "module": "D"}]}, "resolvedFlowVersion": "38.00.000", "flowProperties": [], "typeOfFlow": "Other flow", "classification": {"classHierarchy": "Quantities / Environmental quantities / EPD EN 15804 / LCI indicators", "name": "GaBiCategories"}}, {"dataSetInternalID": 16, "referenceToFlowDataSet": {"shortDescription": [{"value": "Stoffe für die Energierückgewinnung (MER)", "lang": "de"}, {"value": "Materials for energy recovery (MER)", "lang": "en"}], "type": "flow data set", "refObjectId": "59a9181c-3aaf-46ee-8b13-2b3723b6e447", "uri": "../flows/59a9181c-3aaf-46ee-8b13-2b3723b6e447.xml"}, "exchange direction": "OUTPUT", "other": {"anies": [{"name": "referenceToUnitGroupDataSet", "value": {"shortDescription": [{"value": "kg", "lang": "de"}], "type": "unit group data set", "refObjectId": "ad38d542-3fe9-439d-9b95-2f5f7752acaf", "uri": "../unitgroups/ad38d542-3fe9-439d-9b95-2f5f7752acaf.xml"}}, {"value": "0", "module": "A1-A3"}, {"value": "0", "module": "A4"}, {"value": "0", "module": "A5"}, {"value": "0", "module": "C1"}, {"value": "0", "module": "C2"}, {"value": "0", "module": "C3"}, {"value": "0", "module": "C4"}, {"value": "0", "module": "D"}]}, "resolvedFlowVersion": "38.00.000", "flowProperties": [], "typeOfFlow": "Other flow", "classification": {"classHierarchy": "Quantities / Environmental quantities / EPD EN 15804 / LCI indicators", "name": "GaBiCategories"}}, {"dataSetInternalID": 17, "referenceToFlowDataSet": {"shortDescription": [{"value": "Exportierte elektrische Energie (EEE)", "lang": "de"}, {"value": "Exported electrical energy (EEE)", "lang": "en"}], "type": "flow data set", "refObjectId": "4da0c987-2b76-40d6-9e9e-82a017aaaf29", "uri": "../flows/4da0c987-2b76-40d6-9e9e-82a017aaaf29.xml"}, "exchange direction": "OUTPUT", "other": {"anies": [{"name": "referenceToUnitGroupDataSet", "value": {"shortDescription": [{"value": "MJ", "lang": "de"}], "type": "unit group data set", "refObjectId": "93a60a57-a3c8-11da-a746-0800200c9a66", "uri": "../unitgroups/93a60a57-a3c8-11da-a746-0800200c9a66.xml"}}, {"value": "0", "module": "A1-A3"}, {"value": "0", "module": "A4"}, {"value": "0", "module": "A5"}, {"value": "0", "module": "C1"}, {"value": "0", "module": "C2"}, {"value": "0", "module": "C3"}, {"value": "0", "module": "C4"}, {"value": "0", "module": "D"}]}, "resolvedFlowVersion": "38.00.000", "flowProperties": [], "typeOfFlow": "Other flow", "classification": {"classHierarchy": "Quantities / Environmental quantities / EPD EN 15804 / LCI indicators", "name": "GaBiCategories"}}, {"dataSetInternalID": 18, "referenceToFlowDataSet": {"shortDescription": [{"value": "Exportierte thermische Energie (EET)", "lang": "de"}, {"value": "Exported thermal energy (EET)", "lang": "en"}], "type": "flow data set", "refObjectId": "98daf38a-7a79-46d3-9a37-2b7bd0955810", "uri": "../flows/98daf38a-7a79-46d3-9a37-2b7bd0955810.xml"}, "exchange direction": "OUTPUT", "other": {"anies": [{"name": "referenceToUnitGroupDataSet", "value": {"shortDescription": [{"value": "MJ", "lang": "de"}], "type": "unit group data set", "refObjectId": "93a60a57-a3c8-11da-a746-0800200c9a66", "uri": "../unitgroups/93a60a57-a3c8-11da-a746-0800200c9a66.xml"}}, {"value": "0", "module": "A1-A3"}, {"value": "0", "module": "A4"}, {"value": "0", "module": "A5"}, {"value": "0", "module": "C1"}, {"value": "0", "module": "C2"}, {"value": "0", "module": "C3"}, {"value": "0", "module": "C4"}, {"value": "0", "module": "D"}]}, "resolvedFlowVersion": "38.00.000", "flowProperties": [], "typeOfFlow": "Other flow", "classification": {"classHierarchy": "Quantities / Environmental quantities / EPD EN 15804 / LCI indicators", "name": "GaBiCategories"}}]}, "LCIAResults": {"LCIAResult": [{"referenceToLCIAMethodDataSet": {"shortDescription": [{"value": "Globales Erwärmungspotenzial total (GWP-total)", "lang": "de"}, {"value": "Global Warming Potential total (GWP-total)", "lang": "en"}], "type": "LCIA method data set", "refObjectId": "6a37f984-a4b3-458a-a20a-64418c145fa2", "uri": "../lciamethods/6a37f984-a4b3-458a-a20a-64418c145fa2.xml"}, "other": {"anies": [{"name": "referenceToUnitGroupDataSet", "value": {"shortDescription": [{"value": "kg CO_(2)-Äq.", "lang": "de"}], "type": "unit group data set", "refObjectId": "1ebf3012-d0db-4de2-aefd-ef30cedb0be1", "uri": "../unitgroups/1ebf3012-d0db-4de2-aefd-ef30cedb0be1.xml"}}, {"value": "34.7902", "module": "A1-A3"}, {"value": "1.978", "module": "A4"}, {"value": "6.220846", "module": "A5"}, {"value": "0.05440584", "module": "C1"}, {"value": "0.1877", "module": "C2"}, {"value": "1.63115", "module": "C3"}, {"value": "5.96000748", "module": "C4"}, {"value": "-27.632", "module": "D"}]}}, {"referenceToLCIAMethodDataSet": {"shortDescription": [{"value": "Globales Erwärmungspotenzial fossil (GWP-fossil)", "lang": "de"}, {"value": "Global Warming Potential fossil fuels (GWP-fossil)", "lang": "en"}], "type": "LCIA method data set", "refObjectId": "5f635281-343e-44fb-83df-1971b155e6b6", "uri": "../lciamethods/5f635281-343e-44fb-83df-1971b155e6b6.xml"}, "other": {"anies": [{"name": "referenceToUnitGroupDataSet", "value": {"shortDescription": [{"value": "kg CO_(2)-Äq.", "lang": "de"}], "type": "unit group data set", "refObjectId": "1ebf3012-d0db-4de2-aefd-ef30cedb0be1", "uri": "../unitgroups/1ebf3012-d0db-4de2-aefd-ef30cedb0be1.xml"}}, {"value": "39.65", "module": "A1-A3"}, {"value": "1.96", "module": "A4"}, {"value": "0.841", "module": "A5"}, {"value": "0.0544", "module": "C1"}, {"value": "0.186", "module": "C2"}, {"value": "1.63", "module": "C3"}, {"value": "5.96", "module": "C4"}, {"value": "-27.6", "module": "D"}]}}, {"referenceToLCIAMethodDataSet": {"shortDescription": [{"value": "Globales Erwärmungspotenzial biogen (GWP-biogenic)", "lang": "de"}, {"value": "Global Warming Potential biogenic (GWP-biogenic)", "lang": "en"}], "type": "LCIA method data set", "refObjectId": "2356e1ab-0185-4db5-86e5-16de51c7485c", "uri": "../lciamethods/2356e1ab-0185-4db5-86e5-16de51c7485c.xml"}, "other": {"anies": [{"name": "referenceToUnitGroupDataSet", "value": {"shortDescription": [{"value": "kg CO_(2)-Äq.", "lang": "de"}], "type": "unit group data set", "refObjectId": "1ebf3012-d0db-4de2-aefd-ef30cedb0be1", "uri": "../unitgroups/1ebf3012-d0db-4de2-aefd-ef30cedb0be1.xml"}}, {"value": "-5.38", "module": "A1-A3"}, {"value": "0", "module": "A4"}, {"value": "5.38", "module": "A5"}, {"value": "0", "module": "C1"}, {"value": "0", "module": "C2"}, {"value": "0", "module": "C3"}, {"value": "0", "module": "C4"}, {"value": "0", "module": "D"}]}}, {"referenceToLCIAMethodDataSet": {"shortDescription": [{"value": "Globales Erwärmungspotenzial luluc (GWP-luluc)", "lang": "de"}, {"value": "Global Warming Potential luluc (GWP-luluc)", "lang": "en"}], "type": "LCIA method data set", "refObjectId": "4331bbdb-978a-490d-8707-eeb047f01a55", "uri": "../lciamethods/4331bbdb-978a-490d-8707-eeb047f01a55.xml"}, "other": {"anies": [{"name": "referenceToUnitGroupDataSet", "value": {"shortDescription": [{"value": "kg CO_(2)-Äq.", "lang": "de"}], "type": "unit group data set", "refObjectId": "1ebf3012-d0db-4de2-aefd-ef30cedb0be1", "uri": "../unitgroups/1ebf3012-d0db-4de2-aefd-ef30cedb0be1.xml"}}, {"value": "0.5202", "module": "A1-A3"}, {"value": "0.018", "module": "A4"}, {"value": "-0.000154", "module": "A5"}, {"value": "5.84E-06", "module": "C1"}, {"value": "0.0017", "module": "C2"}, {"value": "0.00115", "module": "C3"}, {"value": "7.48E-06", "module": "C4"}, {"value": "-0.032", "module": "D"}]}}, {"referenceToLCIAMethodDataSet": {"shortDescription": [{"value": "Abbau Potential der stratosphärischen Ozonschicht (ODP)", "lang": "de"}, {"value": "Depletion potential of the stratospheric ozone layer (ODP)", "lang": "en"}], "type": "LCIA method data set", "refObjectId": "b5c629d6-def3-11e6-bf01-fe55135034f3", "uri": "../lciamethods/b5c629d6-def3-11e6-bf01-fe55135034f3.xml"}, "other": {"anies": [{"name": "referenceToUnitGroupDataSet", "value": {"shortDescription": [{"value": "kg CFC11-Äq.", "lang": "de"}], "type": "unit group data set", "refObjectId": "d9e957c9-7309-4474-bf3a-7777df6c4e5b", "uri": "../unitgroups/d9e957c9-7309-4474-bf3a-7777df6c4e5b.xml"}}, {"value": "1.061600134E-06", "module": "A1-A3"}, {"value": "1.7E-13", "module": "A4"}, {"value": "-1.32E-11", "module": "A5"}, {"value": "9.92E-13", "module": "C1"}, {"value": "1.6E-14", "module": "C2"}, {"value": "2.75E-11", "module": "C3"}, {"value": "3.81E-13", "module": "C4"}, {"value": "-9.3E-07", "module": "D"}]}}, {"referenceToLCIAMethodDataSet": {"shortDescription": [{"value": "Versauerungspotenzial von Boden und Wasser (AP)", "lang": "de"}, {"value": "Acidification potential of land and water (AP)", "lang": "en"}], "type": "LCIA method data set", "refObjectId": "b5c611c6-def3-11e6-bf01-fe55135034f3", "uri": "../lciamethods/b5c611c6-def3-11e6-bf01-fe55135034f3.xml"}, "other": {"anies": [{"name": "referenceToUnitGroupDataSet", "value": {"shortDescription": [{"value": "mol H^(+)-Äq.", "lang": "de"}], "type": "unit group data set", "refObjectId": "42e089ac-92bf-4bf2-8ca1-5fc40d18f2ed", "uri": "../unitgroups/42e089ac-92bf-4bf2-8ca1-5fc40d18f2ed.xml"}}, {"value": "0.1277", "module": "A1-A3"}, {"value": "0.00213", "module": "A4"}, {"value": "-0.00184", "module": "A5"}, {"value": "0.000115", "module": "C1"}, {"value": "0.00022", "module": "C2"}, {"value": "0.00385", "module": "C3"}, {"value": "0.000569", "module": "C4"}, {"value": "-0.103", "module": "D"}]}}, {"referenceToLCIAMethodDataSet": {"shortDescription": [{"value": "Eutrophierungspotenzial Süßwasser (EP-freshwater)", "lang": "de"}, {"value": "Eutrophication potential aquatic freshwater (EP-freshwater)", "lang": "en"}], "type": "LCIA method data set", "refObjectId": "b53ec18f-7377-4ad3-86eb-cc3f4f276b2b", "uri": "../lciamethods/b53ec18f-7377-4ad3-86eb-cc3f4f276b2b.xml"}, "other": {"anies": [{"name": "referenceToUnitGroupDataSet", "value": {"shortDescription": [{"value": "kg P-Äq.", "lang": "de"}], "type": "unit group data set", "refObjectId": "0429039d-a61d-4590-ba67-aa4a20a810a1", "uri": "../unitgroups/0429039d-a61d-4590-ba67-aa4a20a810a1.xml"}}, {"value": "0.01169958", "module": "A1-A3"}, {"value": "7.07E-06", "module": "A4"}, {"value": "-1.29E-06", "module": "A5"}, {"value": "2.01E-07", "module": "C1"}, {"value": "6.68E-07", "module": "C2"}, {"value": "5.97E-06", "module": "C3"}, {"value": "9.02E-08", "module": "C4"}, {"value": "-0.0104", "module": "D"}]}}, {"referenceToLCIAMethodDataSet": {"shortDescription": [{"value": "Eutrophierungspotenzial Salzwasser (EP-marine)", "lang": "de"}, {"value": "Eutrophication potential aquatic marine (EP-marine)", "lang": "en"}], "type": "LCIA method data set", "refObjectId": "b5c619fa-def3-11e6-bf01-fe55135034f3", "uri": "../lciamethods/b5c619fa-def3-11e6-bf01-fe55135034f3.xml"}, "other": {"anies": [{"name": "referenceToUnitGroupDataSet", "value": {"shortDescription": [{"value": "kg N-Äq.", "lang": "de"}], "type": "unit group data set", "refObjectId": "d05bb823-ecdf-4686-8c40-bf1d9257859f", "uri": "../unitgroups/d05bb823-ecdf-4686-8c40-bf1d9257859f.xml"}}, {"value": "0.049404", "module": "A1-A3"}, {"value": "0.000719", "module": "A4"}, {"value": "-0.000634", "module": "A5"}, {"value": "2.75E-05", "module": "C1"}, {"value": "7.48E-05", "module": "C2"}, {"value": "0.00107", "module": "C3"}, {"value": "0.000161", "module": "C4"}, {"value": "-0.0313", "module": "D"}]}}, {"referenceToLCIAMethodDataSet": {"shortDescription": [{"value": "Eutrophierungspotenzial Land (EP-terrestrial)", "lang": "de"}, {"value": "Eutrophication potential terrestrial (EP-terrestrial)", "lang": "en"}], "type": "LCIA method data set", "refObjectId": "b5c614d2-def3-11e6-bf01-fe55135034f3", "uri": "../lciamethods/b5c614d2-def3-11e6-bf01-fe55135034f3.xml"}, "other": {"anies": [{"name": "referenceToUnitGroupDataSet", "value": {"shortDescription": [{"value": "mol N-Äq.", "lang": "de"}], "type": "unit group data set", "refObjectId": "71b4d617-0ec9-4d3f-b65e-e438940c2401", "uri": "../unitgroups/71b4d617-0ec9-4d3f-b65e-e438940c2401.xml"}}, {"value": "0.35803", "module": "A1-A3"}, {"value": "0.00851", "module": "A4"}, {"value": "-0.00539", "module": "A5"}, {"value": "0.000287", "module": "C1"}, {"value": "0.000904", "module": "C2"}, {"value": "0.0114", "module": "C3"}, {"value": "0.00274", "module": "C4"}, {"value": "-0.253", "module": "D"}]}}, {"referenceToLCIAMethodDataSet": {"shortDescription": [{"value": "Bildungspotential für troposphärisches Ozon (POCP)", "lang": "de"}, {"value": "Formation potential of tropospheric ozone photochemical oxidants (POCP)", "lang": "en"}], "type": "LCIA method data set", "refObjectId": "b5c610fe-def3-11e6-bf01-fe55135034f3", "uri": "../lciamethods/b5c610fe-def3-11e6-bf01-fe55135034f3.xml"}, "other": {"anies": [{"name": "referenceToUnitGroupDataSet", "value": {"shortDescription": [{"value": "kg NMVOC-Äq.", "lang": "de"}], "type": "unit group data set", "refObjectId": "d27c25f8-fbc1-44c6-b47b-4adbae4199c6", "uri": "../unitgroups/d27c25f8-fbc1-44c6-b47b-4adbae4199c6.xml"}}, {"value": "0.73154", "module": "A1-A3"}, {"value": "0.00186", "module": "A4"}, {"value": "-0.00184", "module": "A5"}, {"value": "7.33E-05", "module": "C1"}, {"value": "0.000189", "module": "C2"}, {"value": "0.00287", "module": "C3"}, {"value": "0.00045", "module": "C4"}, {"value": "-0.092", "module": "D"}]}}, {"referenceToLCIAMethodDataSet": {"shortDescription": [{"value": "Potenzial für den abiotischen Abbau nicht fossiler Ressourcen (ADPE)", "lang": "de"}, {"value": "Abiotic depletion potential for non fossil resources (ADPE)", "lang": "en"}], "type": "LCIA method data set", "refObjectId": "b2ad6494-c78d-11e6-9d9d-cec0c932ce01", "uri": "../lciamethods/b2ad6494-c78d-11e6-9d9d-cec0c932ce01.xml"}, "other": {"anies": [{"name": "referenceToUnitGroupDataSet", "value": {"shortDescription": [{"value": "kg Sb-Äq.", "lang": "de"}], "type": "unit group data set", "refObjectId": "54ccd2d9-a32a-4fc2-923d-f2c8c93e89d4", "uri": "../unitgroups/54ccd2d9-a32a-4fc2-923d-f2c8c93e89d4.xml"}}, {"value": "0.0001925987", "module": "A1-A3"}, {"value": "1.25E-07", "module": "A4"}, {"value": "-7.74E-08", "module": "A5"}, {"value": "8.34E-09", "module": "C1"}, {"value": "1.18E-08", "module": "C2"}, {"value": "3.71E-07", "module": "C3"}, {"value": "3.56E-09", "module": "C4"}, {"value": "-0.000164", "module": "D"}]}}, {"referenceToLCIAMethodDataSet": {"shortDescription": [{"value": "Potenzial für den abiotischen Abbau fossiler Brennstoffe (ADPF)", "lang": "de"}, {"value": "Abiotic depletion potential for fossil resources (ADPF)", "lang": "en"}], "type": "LCIA method data set", "refObjectId": "b2ad6110-c78d-11e6-9d9d-cec0c932ce01", "uri": "../lciamethods/b2ad6110-c78d-11e6-9d9d-cec0c932ce01.xml"}, "other": {"anies": [{"name": "referenceToUnitGroupDataSet", "value": {"shortDescription": [{"value": "MJ", "lang": "de"}], "type": "unit group data set", "refObjectId": "93a60a57-a3c8-11da-a746-0800200c9a66", "uri": "../unitgroups/93a60a57-a3c8-11da-a746-0800200c9a66.xml"}}, {"value": "1028.8", "module": "A1-A3"}, {"value": "26.4", "module": "A4"}, {"value": "-53.8", "module": "A5"}, {"value": "1.13", "module": "C1"}, {"value": "2.49", "module": "C2"}, {"value": "33.7", "module": "C3"}, {"value": "0.964", "module": "C4"}, {"value": "-473", "module": "D"}]}}, {"referenceToLCIAMethodDataSet": {"shortDescription": [{"value": "Wassernutzung (WDP)", "lang": "de"}, {"value": "Water use (WDP)", "lang": "en"}], "type": "LCIA method data set", "refObjectId": "b2ad66ce-c78d-11e6-9d9d-cec0c932ce01", "uri": "../lciamethods/b2ad66ce-c78d-11e6-9d9d-cec0c932ce01.xml"}, "other": {"anies": [{"name": "referenceToUnitGroupDataSet", "value": {"shortDescription": [{"value": "m^(3) Welt-Äq. entzogen", "lang": "de"}], "type": "unit group data set", "refObjectId": "6ae2df01-888e-46c8-b17d-49fa3869b476", "uri": "../unitgroups/6ae2df01-888e-46c8-b17d-49fa3869b476.xml"}}, {"value": "8.9896", "module": "A1-A3"}, {"value": "0.0223", "module": "A4"}, {"value": "0.73", "module": "A5"}, {"value": "0.012", "module": "C1"}, {"value": "0.00211", "module": "C2"}, {"value": "0.355", "module": "C3"}, {"value": "0.53", "module": "C4"}, {"value": "-9.66", "module": "D"}]}}, {"referenceToLCIAMethodDataSet": {"shortDescription": [{"value": "Auftreten von Krankheiten aufgrund von Feinstaubemissionen (PM)", "lang": "de"}, {"value": "Incidence of disease due to PM emissions (PM)", "lang": "en"}], "type": "LCIA method data set", "refObjectId": "b5c602c6-def3-11e6-bf01-fe55135034f3", "uri": "../lciamethods/b5c602c6-def3-11e6-bf01-fe55135034f3.xml"}, "other": {"anies": [{"name": "referenceToUnitGroupDataSet", "value": {"shortDescription": [{"value": "Krankheitsfälle", "lang": "de"}], "type": "unit group data set", "refObjectId": "3883559b-648f-4afc-8ba2-0bd24f3affa3", "uri": "../unitgroups/3883559b-648f-4afc-8ba2-0bd24f3affa3.xml"}}, {"module": "A1-A3"}, {"module": "A4"}, {"module": "A5"}, {"module": "C1"}, {"module": "C2"}, {"module": "C3"}, {"module": "C4"}, {"module": "D"}]}}, {"referenceToLCIAMethodDataSet": {"shortDescription": [{"value": "Wirkung durch Exposition des Menschen mit U235 (IR)", "lang": "de"}, {"value": "Human exposure efficiency relative to U235 (IR)", "lang": "en"}], "type": "LCIA method data set", "refObjectId": "b5c632be-def3-11e6-bf01-fe55135034f3", "uri": "../lciamethods/b5c632be-def3-11e6-bf01-fe55135034f3.xml"}, "other": {"anies": [{"name": "referenceToUnitGroupDataSet", "value": {"shortDescription": [{"value": "kBq U235-Äq.", "lang": "de"}], "type": "unit group data set", "refObjectId": "456b05bf-1415-44a9-9993-02452f554c09", "uri": "../unitgroups/456b05bf-1415-44a9-9993-02452f554c09.xml"}}, {"module": "A1-A3"}, {"module": "A4"}, {"module": "A5"}, {"module": "C1"}, {"module": "C2"}, {"module": "C3"}, {"module": "C4"}, {"module": "D"}]}}, {"referenceToLCIAMethodDataSet": {"shortDescription": [{"value": "Toxizitätsvergleichseinheit für Ökosysteme (ETP-fw)", "lang": "de"}, {"value": "Comparative toxic unit for ecosystems (ETP-fw)", "lang": "en"}], "type": "LCIA method data set", "refObjectId": "ee1082d1-b0f7-43ca-a1f0-21e2a4a74511", "uri": "../lciamethods/ee1082d1-b0f7-43ca-a1f0-21e2a4a74511.xml"}, "other": {"anies": [{"name": "referenceToUnitGroupDataSet", "value": {"shortDescription": [{"value": "CTUe", "lang": "de"}], "type": "unit group data set", "refObjectId": "aa959ded-f1eb-4efb-9c5c-2d60be36b3e6", "uri": "../unitgroups/aa959ded-f1eb-4efb-9c5c-2d60be36b3e6.xml"}}, {"module": "A1-A3"}, {"module": "A4"}, {"module": "A5"}, {"module": "C1"}, {"module": "C2"}, {"module": "C3"}, {"module": "C4"}, {"module": "D"}]}}, {"referenceToLCIAMethodDataSet": {"shortDescription": [{"value": "Toxizitätsvergleichseinheit für Menschen (krebserregend) (HTP-c)", "lang": "de"}, {"value": "Comparative toxic unit for humans (carcinogenic) (HTP-c)", "lang": "en"}], "type": "LCIA method data set", "refObjectId": "2299222a-bbd8-474f-9d4f-4dd1f18aea7c", "uri": "../lciamethods/2299222a-bbd8-474f-9d4f-4dd1f18aea7c.xml"}, "other": {"anies": [{"name": "referenceToUnitGroupDataSet", "value": {"shortDescription": [{"value": "CTUh", "lang": "de"}], "type": "unit group data set", "refObjectId": "d4c9523e-2d7e-49fd-8469-998f547d3a70", "uri": "../unitgroups/d4c9523e-2d7e-49fd-8469-998f547d3a70.xml"}}, {"module": "A1-A3"}, {"module": "A4"}, {"module": "A5"}, {"module": "C1"}, {"module": "C2"}, {"module": "C3"}, {"module": "C4"}, {"module": "D"}]}}, {"referenceToLCIAMethodDataSet": {"shortDescription": [{"value": "Toxizitätsvergleichseinheit für Menschen (nicht krebserregend) (HTP-nc)", "lang": "de"}, {"value": "Comparative toxic unit for humans (noncarcinogenic) (HTP-nc)", "lang": "en"}], "type": "LCIA method data set", "refObjectId": "3af763a5-b7a1-48c9-9cee-1f223481fcef", "uri": "../lciamethods/3af763a5-b7a1-48c9-9cee-1f223481fcef.xml"}, "other": {"anies": [{"name": "referenceToUnitGroupDataSet", "value": {"shortDescription": [{"value": "CTUh", "lang": "de"}], "type": "unit group data set", "refObjectId": "d4c9523e-2d7e-49fd-8469-998f547d3a70", "uri": "../unitgroups/d4c9523e-2d7e-49fd-8469-998f547d3a70.xml"}}, {"module": "A1-A3"}, {"module": "A4"}, {"module": "A5"}, {"module": "C1"}, {"module": "C2"}, {"module": "C3"}, {"module": "C4"}, {"module": "D"}]}}, {"referenceToLCIAMethodDataSet": {"shortDescription": [{"value": "Bodenqualitätsindex (SQP)", "lang": "de"}, {"value": "Soil quality index (SQP)", "lang": "en"}], "type": "LCIA method data set", "refObjectId": "b2ad6890-c78d-11e6-9d9d-cec0c932ce01", "uri": "../lciamethods/b2ad6890-c78d-11e6-9d9d-cec0c932ce01.xml"}, "other": {"anies": [{"name": "referenceToUnitGroupDataSet", "value": {"shortDescription": [{"value": "SQP", "lang": "de"}], "type": "unit group data set", "refObjectId": "f130951c-e67f-4f7f-8dd4-665de3974e18", "uri": "../unitgroups/f130951c-e67f-4f7f-8dd4-665de3974e18.xml"}}, {"module": "A1-A3"}, {"module": "A4"}, {"module": "A5"}, {"module": "C1"}, {"module": "C2"}, {"module": "C3"}, {"module": "C4"}, {"module": "D"}]}}]}, "otherAttributes": {"{http://www.indata.network/EPD/2019}epd-version": "1.2"}, "version": "1.1", "locations": "../ILCDLocations.xml"}