{"processInformation": {"dataSetInformation": {"UUID": "7ee2591b-29a8-4e2e-9fdc-09f9ad2630e6", "name": {"baseName": [{"value": "STS Carpet Tile with Nylon Face Fibre", "lang": "en"}, {"value": "STS Carpet Tile with Nylon Face Fibre", "lang": "de"}], "functionalUnitFlowProperties": [{"lang": "en"}]}, "classificationInformation": {"classification": [{"class": [{"value": "Kunststoffe", "level": 0, "classId": "6"}, {"value": "Bodenbeläge", "level": 1, "classId": "6.2"}, {"value": "Mehrschichtig modulare Bodenbeläge", "level": 2, "classId": "6.2.06"}], "name": "OEKOBAU.DAT"}, {"class": [{"value": "02 Building products", "level": 0}, {"value": "Floor coverings", "level": 1}, {"value": "Floor coverings", "level": 2}], "name": "IBUCategories"}]}, "generalComment": [{"value": "This EPD applies to STS Premium Loop Pile Tufted, Bitumen Backed Carpet Tile with Nylon face fibre.\n\nThe carpet tile backing system contains a modified bitumen polymer, mineral filler, and a fibreglass reinforcement layer for dimensional stability. The face fibre is made of solution-dyed Nylon that is tufted into a primary backing sheet, then latex is added to anchor the fibre in place to assure maximum tuft bind. The bitumen-based backing system is then applied to create a durable flooring solution for use in varied applications. The carpet tiles are then die-cut and packaged for distribution.\n\nThis STS Premium Loop Pile Tufted, Bitumen Backed Carpet Tile is a commercial carpet tile, suitable for use in all commercial settings as a floor covering, in accordance with manufacturer guidelines. It has a life span of 10 years and comes with a 10-year wear warranty (subject only to installation and maintenance being carried out in line with manufacturer's guidelines). The product meets both internal and external performance standards including those established in the EU under EN 1307 and EN 10874 for a product suitable for heavy and general commercial installations.\n\nSTS Premium Loop Pile Tufted, Bitumen Backed Carpet Tile comes in various styles. All styles have the same raw material formulation but different designs.\n\nThis product is manufactured in the UK in ISO 9001- and ISO 14001-certified facilities, or equivalent. Raw materials are responsibly sourced through supply chain, chemical and waste management programs. No co-products are produced in the manufacturing of these premium carpet tiles. \n\nDetailed Product Descriptions:", "lang": "en"}, {"value": "Diese EPD gilt für STS Premium Loop Pile Tufted, Bitumen-Rückenbeschichtung mit Nylon-Deckschicht. Das Rückenbeschichtungssystem für Teppichfliesen enthält ein modifiziertes Bitumenpolymer, mineralischen Füllstoff und eine Glasfaser-Verstärkungsschicht für Dimensionsstabilität. Die Deckschicht besteht aus lösungsgefärbtem Nylon, das in eine primäre Trägerbahn getuftet wird. Anschließend wird Latex hinzugefügt, um die Faser zu verankern und eine maximale Tuftbindung zu gewährleisten. Anschließend wird das Rückensystem auf Bitumenbasis aufgebracht, um eine dauerhafte Bodenbelagslösung für verschiedene Anwendungen zu schaffen. Die Teppichfliesen werden dann gestanzt und für den Vertrieb verpackt. Diese STS Premium Loop Pile Tufted, Bitumen Backed Carpet Tile ist eine Teppichfliese für den gewerblichen Einsatz, die gemäß den Richtlinien des Herstellers in allen gewerblichen Bereichen als Bodenbelag verwendet werden kann. Sie hat eine Lebensdauer von 12 Jahren und wird mit einer 12-jährigen Abnutzungsgarantie geliefert (unter der Voraussetzung, dass Verlegung und Pflege gemäß den Richtlinien des Herstellers durchgeführt werden). Das Produkt erfüllt sowohl interne als auch externe Leistungsstandards, einschließlich der in der EU unter EN 1307 und EN 10874 festgelegten Standards für ein Produkt, das für schwere und allgemeine gewerbliche Installationen geeignet ist. Dieses Produkt wird in Großbritannien in ISO 9001- und ISO 14001-zertifizierten Einrichtungen oder gleichwertigen Einrichtungen hergestellt. Die Rohstoffe werden im Rahmen von Programmen für die Lieferkette, das Chemikalien- und das Abfallmanagement verantwortungsvoll beschafft. Bei der Herstellung dieser hochwertigen Teppichfliesen werden keine Nebenprodukte erzeugt. \n\nDetaillierte Produktbeschreibungen: Urban Myth ist ein texturierter Schlingenpolteppich, der sowohl als Fliese als auch als Planke erhältlich ist. Das zufällige Design bietet Vielseitigkeit und die Möglichkeit, innovative und komplementäre Farben zu kreieren, bestehend aus sechs grauen Grundtönen und sechs leuchtenden Akzentfarben, die zu atemberaubenden Installationen kombiniert werden können. Lunar ist eine getuftete Teppichfliese mit Schlingenflor. Inspiriert von der Mondlandschaft ist das Design in acht verschiedenen Farben erhältlich, um eine stilvolle und moderne Umgebung zu schaffen. Lunar eignet sich für eine Vielzahl von Anwendungen, darunter auch für Büros und Bildungseinrichtungen. Cityscene & Brickworks sind getuftete Schlingenteppichfliesen, die zusammen verwendet werden können, um interessante und moderne Bodenbeläge zu schaffen. Sie können auch mit Emphasis kombiniert werden, um ein einzigartiges Design-Statement zu schaffen. Sie eignen sich für eine Vielzahl von Einsatzbereichen, darunter Büros, Bildungseinrichtungen und das Gesundheitswesen.", "lang": "de"}]}, "quantitativeReference": {"referenceToReferenceFlow": [0]}, "time": {"referenceYear": 2023, "dataSetValidUntil": 2028, "other": {"anies": [{"name": "publicationDateOfEPD", "value": 1702857600000}]}}, "geography": {"locationOfOperationSupplyOrProduction": {"location": "RER"}}, "technology": {"technologyDescriptionAndIncludedProcesses": [{"value": "This EPD applies to STS Premium Loop Pile Tufted, Bitumen Backed Carpet Tile with Nylon face fibre. The carpet tile backing system contains a modified bitumen polymer, mineral filler, and a fibreglass reinforcement layer for dimensional stability. The face fibre is made of solution-dyed Nylon that is tufted into a primary backing sheet, then latex is added to anchor the fibre in place to assure maximum tuft bind. The bitumen-based backing system is then applied to create a durable flooring solution for use in varied applications. The carpet tiles are then die-cut and packaged for distribution. \nTechnical data: \nThe technical specifications of the product are listed on the products specification sheet, found at STSorders@sanquhartilesltd.co.uk. This product meets the requirements of the harmonized European Norm (hEN): EN14041:2004A/C:2006. Declarations of performance related to fire, electrostatic, formaldehyde emissions, and slip resistance can be found on the products specification sheet. \nDeclared unit: \nThe declaration refers to the declared unit of 1 m of installed carpet tile.", "lang": "en"}, {"value": "Diese EPD gilt für STS Premium Loop Pile Tufted, Teppichfliesen mit Bitumenrücken und Nylon-Deckschicht.\n\nDas Rückensystem der Teppichfliese enthält ein modifiziertes Bitumenpolymer, einen mineralischen Füllstoff und eine Glasfaserverstärkungsschicht für die Dimensionsstabilität. Die Deckfaser besteht aus lösungsgefärbtem Nylon, das in eine primäre Trägerbahn getuftet wird. Anschließend wird Latex hinzugefügt, um die Faser an ihrem Platz zu verankern und eine maximale Tuftbindung zu gewährleisten. Anschließend wird das Rückensystem auf Bitumenbasis aufgebracht, um eine dauerhafte Bodenbelagslösung für verschiedene Anwendungen zu schaffen. Die Teppichfliesen werden dann gestanzt und für den Vertrieb verpackt. \nTechnische Daten: \nDie technischen Daten des Produkts sind auf dem Produktdatenblatt aufgeführt, das Sie unter www.shawcontract.com finden. Dieses Produkt erfüllt die Anforderungen der harmonisierten europäischen Norm (hEN): EN14041:2004A/C:2006. Leistungserklärungen in Bezug auf Feuer, Elektrostatik, Formaldehyd-Emissionen und Rutschfestigkeit finden Sie auf dem Produktdatenblatt.   \nDeklarierte Einheit: \nDie Deklaration bezieht sich auf die deklarierte Einheit von 1 m² verlegter Teppichfliese.", "lang": "de"}], "technologicalApplicability": [{"value": "STS Premium Loop Pile Tufted, Bitumen Backed Carpet Tile with Nylon Face Fibre is suitable for use as a floor covering in heavy and general commercial installations.", "lang": "en"}, {"value": "STS Premium Loop Pile Tufted, Bitumen Backed Carpet Tile mit Nylon Face Fibre eignet sich für die Verwendung als Bodenbelag in schweren und allgemeinen gewerblichen Installationen.", "lang": "de"}]}}, "modellingAndValidation": {"LCIMethodAndAllocation": {"typeOfDataSet": "EPD", "referenceToLCAMethodDetails": [{"shortDescription": [{"value": "Floor coverings.pdf", "lang": "en"}], "type": "source data set", "refObjectId": "a384d398-e689-45af-b9c8-b4bffb1e2f4e"}], "other": {"anies": [{"name": "subType", "value": "specific dataset"}]}}, "dataSourcesTreatmentAndRepresentativeness": {"referenceToDataSource": [{"shortDescription": [{"value": "GaBi Database (all versions)", "lang": "en"}], "type": "source data set", "refObjectId": "28d74cc0-db8b-4d7e-bc44-5f6d56ce0c4a"}, {"shortDescription": [{"value": "GaBi Database Edition 2022, CUP 2022.02", "lang": "en"}], "type": "source data set", "refObjectId": "94f442cb-662e-43ea-a792-4b0a35132e93"}], "useAdviceForDataSet": [{"value": "Scope: \nA Life Cycle Assessment (LCA) was conducted based upon production data collected from STS, Plant SQ manufacturing facility (Blackaddie Road, Sanquhar, DG46DB), located in Scotland, UK. Production data was collected for STS Premium Loop Pile Tufted, Bitumen Backed Carpet Tile with Nylon Face Fibre, for the period of one year, from January to December 2021.\n\nThis EPD is cradle-to-gate with options in scope with additional modules A4, A5, B1 and B2. The EPD is created in accordance to the specifications of EN 15804+A2.\n\nThe functional unit has been defined as 1 m2 of installed STS Premium Loop Pile Tufted, Bitumen Backed Carpet Tile.\n\nThe EPD was generated with the help of Envision LCA Tool, version 1. The tool has not been manipulated in calculating impact results. The current version of the tool is maintained, saved, and stored for 10 years to be used for revision and re-traceability purposes. \nSystem boundary: \nThe type of EPD is Cradle-to-Gate with options modules C1– C4, module D, and additional modules. The additional modules are A4, A5, B1 and B2.\n\nThe modules considered in the life cycle assessment and environmental product declaration, based on the products entire life cycle, are described as follows:\n\nProduction Stage:  \n\nModule A1 - Provision of Raw Materials.\nModule A2 - Transport of Raw Materials.\nModule A3 - Manufacturing.Construction/Installation Stage:\n\nModule A4 - Transportation by truck of the product to the construction site in Europe. \nModule A5 - Installation of the carpet, treatment of cutting waste (landfill) and packaging waste (landfill, recycling, and incineration). The production of the amount of carpet that occurs as installation waste is also included along with its transport to the place of installation. Biogenic carbon that is stored in the wooden pallets and cardboard (packaging) is released as carbon dioxide emissions into the air at the end of life in module A5.Use Stage:\n\nModule B1 - Indoor emissions of volatile organic compounds (VOCs) during the first few months after installation.\nModule B2 - Carpet cleaning per year, including vacuuming (electricity consumption) and hot water cleaning (electricity and water consumption, as well as waste water treatment).\nModule B3 - Repair (module not relevant).\nModule B4 - Replacement (module not relevant).\nModule B5 - Refurbishment (module not relevant).\nModule B6 - Operational Energy Use (module not relevant).\nModule B7 - Operational Water Use (module not relevant).End of Life Stage:\nThree scenarios have been evaluated:\nScenario 1: the STS Bitumen Backed carpet is 100% disposed of in a landfill.\nScenario 2: the STS Bitumen Backed carpet is 100% incinerated. \nScenario 3: 40% of STS Bitumen Backed carpets are incinerated and the remaining 60% are landfilled. This assumption is based on the carpet disposal rates in Europe mentioned in the study conducted by Deutsche Umwelthilfe in 2017 (Umwelthilfe, 2017) and the European Commission in 2013 (Commission, 2013).\n\nModule C1 - The carpet is de-constructed manually and no additional environmental impact is caused.\nModule C2 - Transport of the carpet waste to a landfill or to the municipal waste incineration plant.\nModule C3 - Impacts from thermal treatment disposal (C3/2 and C3/3).\nModule C4 - Impacts from landfill disposal (C4/1 and C4/3).Module D includes benefits from energy recovery via treatment of packaging materials and incineration of carpets at their end of life (D/1, D/2 and D/3), as well as the burdens of balancing the secondary material content in modules A1 and A3 via the net-scrap approach.", "lang": "en"}, {"value": "Gültigkeitsbereich: \nEine Ökobilanz (LCA) wurde auf der Grundlage von Produktionsdaten durchgeführt, die von Shaw Contract (Shaw Europe, Ltd.), Werk SQ (Blackaddie Road, Sanquhar, DG46DB), in Schottland, Großbritannien, gesammelt wurden. Die Produktionsdaten wurden für STS Premium Loop Pile Tufted, Bitumen Backed Carpet Tile with Nylon Face Fibre für den Zeitraum von einem Jahr, von Januar bis Dezember 2021, erhoben. Diese EPD umfasst alle Module von der Wiege bis zur Bahre und wurde in Übereinstimmung mit den Spezifikationen der EN 15804+A2 erstellt. Die funktionelle Einheit wurde als 1 m2 STS Premium Loop Pile Tufted, Bitumen Backed Carpet Tile definiert. \nSystemgrenze: \nDer Typ der EPD ist Cradle-to-Grave.\n\nDie in der Ökobilanz und der Umweltproduktdeklaration berücksichtigten Module, die auf dem gesamten Lebenszyklus des Produkts basieren, werden wie folgt beschrieben: Produktionsphase: Modul A1 - Bereitstellung von Rohstoffen Modul A2 - Transport von Rohstoffen Modul A3 - HerstellungBau-/Installationsphase: Modul A4 - Transport zur Baustelle Modul A5 - Montage-/Installationsverluste, einschließlich VerpackungsmaterialNutzungsphase:\n\nModul B1 - Produktnutzung/Emissionen Modul B2 - Produktwartung Modul B3 - Reparatur (Modul nicht relevant) Modul B4 - Ersatz (Modul nicht relevant) Modul B5 - Aufarbeitung (Modul nicht relevant) Modul B6 - Betrieblicher Energieverbrauch (Modul nicht relevant) Modul B7 - Betrieblicher Wasserverbrauch (Modul nicht relevant) End-of-Life-Stadium: Modul C1 - Abriss/manuelle Demontage Modul C2 - Transport zur Entsorgungsstelle Modul C3 - Abfallverarbeitung (ohne Auswirkungen deklariert) Modul C4 - EntsorgungModul D umfasst Wiederverwendungs-, Verwertungs- und/oder Recyclingpotenzial. Die Gutschriften außerhalb der Systemgrenze werden berücksichtigt.", "lang": "de"}], "other": {"anies": [{"name": "referenceToOriginalEPD", "value": {"shortDescription": {"value": "STS Carpet Tile with Nylon Face Fibre.pdf", "defaultValue": "STS Carpet Tile with Nylon Face Fibre.pdf", "lstrings": [{"lang": "en", "value": "STS Carpet Tile with Nylon Face Fibre.pdf"}]}, "type": "source data set", "uuid": {"uuid": "bdf259ff-d5c9-4fd0-beb9-bfe64b15f292"}, "refObjectId": "bdf259ff-d5c9-4fd0-beb9-bfe64b15f292", "resourceURLs": ["https://oekobaudat.de/OEKOBAU.DAT/resource/sources/bdf259ff-d5c9-4fd0-beb9-bfe64b15f292/STS_Carpet_Tile_with_Nylon_Face_Fibre_19669.pdf?version=00.06.000"]}}]}}, "validation": {"review": [{"referenceToNameOfReviewerAndInstitution": [{"shortDescription": [{"value": "Institut Bauen und Umwelt e. V.", "lang": "en"}], "type": "contact data set", "refObjectId": "d111dbec-b024-4be5-86c5-752d6eb2cf95", "uri": "../contacts/d111dbec-b024-4be5-86c5-752d6eb2cf95.xml"}], "type": "Accredited third party review"}]}, "complianceDeclarations": {"compliance": [{"referenceToComplianceSystem": {"shortDescription": [{"value": "DIN EN 15804+A2", "lang": "en"}], "type": "source data set", "refObjectId": "c0016b33-8cf7-415c-ac6e-deba0d21440d", "uri": "../sources/c0016b33-8cf7-415c-ac6e-deba0d21440d.xml"}}, {"referenceToComplianceSystem": {"shortDescription": [{"value": "ISO 14025", "lang": "en"}], "type": "source data set", "refObjectId": "4f2eb655-6e44-4874-a95a-e28f5442cd4d", "uri": "../sources/4f2eb655-6e44-4874-a95a-e28f5442cd4d.xml"}}]}}, "administrativeInformation": {"commissionerAndGoal": {"referenceToCommissioner": [{"shortDescription": [{"value": "STS", "lang": "en"}], "type": "contact data set", "refObjectId": "98311727-f008-4777-9673-cde8976e9881", "uri": "../contacts/98311727-f008-4777-9673-cde8976e9881.xml"}]}, "dataGenerator": {"referenceToPersonOrEntityGeneratingTheDataSet": [{"shortDescription": [{"value": "Sphera Solutions GmbH", "lang": "en"}], "type": "contact data set", "refObjectId": "623edf96-39d1-4e6f-9892-674c7228546b", "uri": "../contacts/623edf96-39d1-4e6f-9892-674c7228546b.xml"}]}, "dataEntryBy": {"timeStamp": 1702857600000, "referenceToDataSetFormat": [{"shortDescription": [{"value": "ILCD Format", "lang": "en"}], "type": "source data set", "refObjectId": "a97a0155-0234-4b87-b4ce-a45da52f2a40", "uri": "../sources/a97a0155-0234-4b87-b4ce-a45da52f2a40.xml"}, {"shortDescription": [{"value": "EPD-Datenformaterweiterungen v1.2", "lang": "de"}, {"value": "EPD Data Format Extensions v1.2", "lang": "en"}], "type": "source data set", "refObjectId": "a29449fd-aa2f-4de8-b5d7-4b06b43c6fde", "uri": "../sources/a29449fd-aa2f-4de8-b5d7-4b06b43c6fde.xml"}]}, "publicationAndOwnership": {"dataSetVersion": "00.09.000", "referenceToRegistrationAuthority": {"shortDescription": [{"value": "Institut Bauen und Umwelt e. V.", "lang": "en"}], "type": "contact data set", "refObjectId": "d111dbec-b024-4be5-86c5-752d6eb2cf95", "uri": "../contacts/d111dbec-b024-4be5-86c5-752d6eb2cf95.xml"}, "registrationNumber": "EPD-SHA-20230445-CBA6-EN", "referenceToOwnershipOfDataSet": {"shortDescription": [{"value": "STS", "lang": "en"}], "type": "contact data set", "refObjectId": "98311727-f008-4777-9673-cde8976e9881", "uri": "../contacts/98311727-f008-4777-9673-cde8976e9881.xml"}, "copyright": true, "licenseType": "Free of charge for all users and uses", "accessRestrictions": [{"value": "None", "lang": "en"}], "other": {"anies": [{"name": "referenceToPublisher", "value": {"shortDescription": [{"value": "Institut Bauen und Umwelt e. V.", "lang": "en"}], "type": "contact data set", "refObjectId": "d111dbec-b024-4be5-86c5-752d6eb2cf95", "uri": "../contacts/d111dbec-b024-4be5-86c5-752d6eb2cf95.xml"}}]}}}, "exchanges": {"exchange": [{"dataSetInternalID": 0, "referenceToFlowDataSet": {"shortDescription": [{"value": "STS Bitumen Backed Carpet (STS Carpet Tile with Nylon Face Fibre)", "lang": "en"}], "type": "flow data set", "refObjectId": "6c8e7992-e462-7b63-5d9e-bde41c9dd24e", "uri": "../flows/6c8e7992-e462-7b63-5d9e-bde41c9dd24e.xml"}, "meanAmount": 1.0, "referencesToDataSource": {}, "referenceFlow": true, "resolvedFlowVersion": "00.08.000", "resultingflowAmount": 1.0, "flowProperties": [{"name": [{"lang": "en", "value": "Area"}, {"lang": "de", "value": "Fläche"}], "uuid": "93a60a56-a3c8-19da-a746-0800200c9a66", "referenceFlowProperty": true, "meanValue": 1.0, "referenceUnit": "qm", "unitGroupUUID": "c20a03d7-bd90-4569-bc94-66cfd364dfc8"}], "materialProperties": [{"name": "layer thickness", "value": "0.006", "unit": "m", "unitDescription": "meters"}, {"name": "grammage", "value": "3.896", "unit": "kg/m^2", "unitDescription": "kilograms per square meter"}], "typeOfFlow": "Product flow", "classification": {"classHierarchy": "Kunststoffe / Bodenbeläge / Mehrschichtig modulare Bodenbeläge", "name": "OEKOBAU.DAT"}}, {"dataSetInternalID": 1, "referenceToFlowDataSet": {"shortDescription": [{"value": "Renewable primary energy as energy carrier (PERE)", "lang": "en"}, {"value": "Erneuerbare Primärenergie als Energieträger (PERE)", "lang": "de"}], "type": "flow data set", "refObjectId": "20f32be5-0398-4288-9b6d-accddd195317", "uri": "../flows/20f32be5-0398-4288-9b6d-accddd195317.xml"}, "exchange direction": "INPUT", "other": {"anies": [{"name": "referenceToUnitGroupDataSet", "value": {"shortDescription": [{"value": "MJ", "lang": "en"}], "type": "unit group data set", "refObjectId": "93a60a57-a3c8-11da-a746-0800200c9a66", "uri": "../unitgroups/93a60a57-a3c8-11da-a746-0800200c9a66.xml"}}, {"value": "12.1049867927783", "module": "A1-A3"}, {"value": "0.195032970205839", "module": "A4"}, {"value": "5.11000231486595", "module": "A5"}, {"value": "0", "module": "B1"}, {"value": "2.30542568779605", "module": "B2"}, {"value": "0", "module": "C1"}, {"value": "0.0399436271478983", "module": "C2"}, {"value": "0", "module": "C3"}, {"value": "0.322130368038554", "module": "C4"}, {"value": "-0.129048096452913", "module": "D"}]}, "resolvedFlowVersion": "38.00.000", "flowProperties": [], "typeOfFlow": "Other flow", "classification": {"classHierarchy": "Quantities", "name": "GaBiCategories"}}, {"dataSetInternalID": 2, "referenceToFlowDataSet": {"shortDescription": [{"value": "Renewable primary energy resources as material utilization (PERM)", "lang": "en"}, {"value": "Erneuerbare Primärenergie zur stofflichen Nutzung (PERM)", "lang": "de"}], "type": "flow data set", "refObjectId": "fb3ec0de-548d-4508-aea5-00b73bf6f702", "uri": "../flows/fb3ec0de-548d-4508-aea5-00b73bf6f702.xml"}, "exchange direction": "INPUT", "other": {"anies": [{"name": "referenceToUnitGroupDataSet", "value": {"shortDescription": [{"value": "MJ", "lang": "en"}], "type": "unit group data set", "refObjectId": "93a60a57-a3c8-11da-a746-0800200c9a66", "uri": "../unitgroups/93a60a57-a3c8-11da-a746-0800200c9a66.xml"}}, {"value": "5.306440264", "module": "A1-A3"}, {"value": "0", "module": "A4"}, {"value": "-4.188556345342", "module": "A5"}, {"value": "0", "module": "B1"}, {"value": "0", "module": "B2"}, {"value": "0", "module": "C1"}, {"value": "0", "module": "C2"}, {"value": "0", "module": "C3"}, {"value": "0", "module": "C4"}, {"value": "0", "module": "D"}]}, "resolvedFlowVersion": "38.00.000", "flowProperties": [], "typeOfFlow": "Other flow", "classification": {"classHierarchy": "Quantities", "name": "GaBiCategories"}}, {"dataSetInternalID": 3, "referenceToFlowDataSet": {"shortDescription": [{"value": "Total use of renewable primary energy resources (PERT)", "lang": "en"}, {"value": "Total erneuerbare Primärenergie (PERT)", "lang": "de"}], "type": "flow data set", "refObjectId": "53f97275-fa8a-4cdd-9024-65936002acd0", "uri": "../flows/53f97275-fa8a-4cdd-9024-65936002acd0.xml"}, "exchange direction": "INPUT", "other": {"anies": [{"name": "referenceToUnitGroupDataSet", "value": {"shortDescription": [{"value": "MJ", "lang": "en"}], "type": "unit group data set", "refObjectId": "93a60a57-a3c8-11da-a746-0800200c9a66", "uri": "../unitgroups/93a60a57-a3c8-11da-a746-0800200c9a66.xml"}}, {"value": "17.4114270567783", "module": "A1-A3"}, {"value": "0.195032970205839", "module": "A4"}, {"value": "0.921445969523948", "module": "A5"}, {"value": "0", "module": "B1"}, {"value": "2.30542568779605", "module": "B2"}, {"value": "0", "module": "C1"}, {"value": "0.0399436271478983", "module": "C2"}, {"value": "0", "module": "C3"}, {"value": "0.322130368038554", "module": "C4"}, {"value": "-0.129048096452913", "module": "D"}]}, "resolvedFlowVersion": "38.00.000", "flowProperties": [], "typeOfFlow": "Other flow", "classification": {"classHierarchy": "Quantities / Environmental quantities / EPD EN 15804 / LCI indicators", "name": "GaBiCategories"}}, {"dataSetInternalID": 4, "referenceToFlowDataSet": {"shortDescription": [{"value": "Non renewable primary energy as energy carrier (PENRE)", "lang": "en"}, {"value": "Nicht-erneuerbare Primärenergie als Energieträger (PENRE)", "lang": "de"}], "type": "flow data set", "refObjectId": "ac857178-2b45-46ec-892a-a9a4332f0372", "uri": "../flows/ac857178-2b45-46ec-892a-a9a4332f0372.xml"}, "exchange direction": "INPUT", "other": {"anies": [{"name": "referenceToUnitGroupDataSet", "value": {"shortDescription": [{"value": "MJ", "lang": "en"}], "type": "unit group data set", "refObjectId": "93a60a57-a3c8-11da-a746-0800200c9a66", "uri": "../unitgroups/93a60a57-a3c8-11da-a746-0800200c9a66.xml"}}, {"value": "131.272572847431", "module": "A1-A3"}, {"value": "3.43893828498179", "module": "A4"}, {"value": "1.5723700015066", "module": "A5"}, {"value": "0", "module": "B1"}, {"value": "4.15443268399767", "module": "B2"}, {"value": "0", "module": "C1"}, {"value": "0.704309986639546", "module": "C2"}, {"value": "0", "module": "C3"}, {"value": "3.92027696824413", "module": "C4"}, {"value": "-0.501948366711921", "module": "D"}]}, "resolvedFlowVersion": "38.00.000", "flowProperties": [], "typeOfFlow": "Other flow", "classification": {"classHierarchy": "Quantities", "name": "GaBiCategories"}}, {"dataSetInternalID": 5, "referenceToFlowDataSet": {"shortDescription": [{"value": "Non renewable primary energy as material utilization (PENRM)", "lang": "en"}, {"value": "Nicht-erneuerbare Primärenergie zur stofflichen Nutzung (PENRM)", "lang": "de"}], "type": "flow data set", "refObjectId": "1421caa0-679d-4bf4-b282-0eb850ccae27", "uri": "../flows/1421caa0-679d-4bf4-b282-0eb850ccae27.xml"}, "exchange direction": "INPUT", "other": {"anies": [{"name": "referenceToUnitGroupDataSet", "value": {"shortDescription": [{"value": "MJ", "lang": "en"}], "type": "unit group data set", "refObjectId": "93a60a57-a3c8-11da-a746-0800200c9a66", "uri": "../unitgroups/93a60a57-a3c8-11da-a746-0800200c9a66.xml"}}, {"value": "51.0401506982", "module": "A1-A3"}, {"value": "0", "module": "A4"}, {"value": "-0.316781634121", "module": "A5"}, {"value": "0", "module": "B1"}, {"value": "0", "module": "B2"}, {"value": "0", "module": "C1"}, {"value": "0", "module": "C2"}, {"value": "0", "module": "C3"}, {"value": "0", "module": "C4"}, {"value": "0", "module": "D"}]}, "resolvedFlowVersion": "38.00.000", "flowProperties": [], "typeOfFlow": "Other flow", "classification": {"classHierarchy": "Quantities", "name": "GaBiCategories"}}, {"dataSetInternalID": 6, "referenceToFlowDataSet": {"shortDescription": [{"value": "Total use of non renewable primary energy resources (PENRT)", "lang": "en"}, {"value": "Total nicht erneuerbare Primärenergie (PENRT)", "lang": "de"}], "type": "flow data set", "refObjectId": "06159210-646b-4c8d-8583-da9b3b95a6c1", "uri": "../flows/06159210-646b-4c8d-8583-da9b3b95a6c1.xml"}, "exchange direction": "INPUT", "other": {"anies": [{"name": "referenceToUnitGroupDataSet", "value": {"shortDescription": [{"value": "MJ", "lang": "en"}], "type": "unit group data set", "refObjectId": "93a60a57-a3c8-11da-a746-0800200c9a66", "uri": "../unitgroups/93a60a57-a3c8-11da-a746-0800200c9a66.xml"}}, {"value": "180.641186272744", "module": "A1-A3"}, {"value": "3.43893828498179", "module": "A4"}, {"value": "1.2555883673856", "module": "A5"}, {"value": "0", "module": "B1"}, {"value": "4.1544326839977", "module": "B2"}, {"value": "0", "module": "C1"}, {"value": "0.704309986639546", "module": "C2"}, {"value": "0", "module": "C3"}, {"value": "3.92027696824416", "module": "C4"}, {"value": "-0.501948366711923", "module": "D"}]}, "resolvedFlowVersion": "38.00.000", "flowProperties": [], "typeOfFlow": "Other flow", "classification": {"classHierarchy": "Quantities / Environmental quantities / EPD EN 15804 / LCI indicators", "name": "GaBiCategories"}}, {"dataSetInternalID": 7, "referenceToFlowDataSet": {"shortDescription": [{"value": "Use of secondary material (SM)", "lang": "en"}, {"value": "Einsatz von Sekundärstoffen (SM)", "lang": "de"}], "type": "flow data set", "refObjectId": "c6a1f35f-2d09-4f54-8dfb-97e502e1ce92", "uri": "../flows/c6a1f35f-2d09-4f54-8dfb-97e502e1ce92.xml"}, "exchange direction": "INPUT", "other": {"anies": [{"name": "referenceToUnitGroupDataSet", "value": {"shortDescription": [{"value": "kg", "lang": "en"}], "type": "unit group data set", "refObjectId": "ad38d542-3fe9-439d-9b95-2f5f7752acaf", "uri": "../unitgroups/ad38d542-3fe9-439d-9b95-2f5f7752acaf.xml"}}, {"value": "0.109635051415221", "module": "A1-A3"}, {"value": "0", "module": "A4"}, {"value": "0.00577026586395898", "module": "A5"}, {"value": "0", "module": "B1"}, {"value": "0", "module": "B2"}, {"value": "0", "module": "C1"}, {"value": "0", "module": "C2"}, {"value": "0", "module": "C3"}, {"value": "0", "module": "C4"}, {"value": "-0.11540531727918", "module": "D"}]}, "resolvedFlowVersion": "38.00.000", "flowProperties": [], "typeOfFlow": "Other flow", "classification": {"classHierarchy": "Quantities / Environmental quantities / EPD EN 15804 / LCI indicators", "name": "GaBiCategories"}}, {"dataSetInternalID": 8, "referenceToFlowDataSet": {"shortDescription": [{"value": "Use of renewable secondary fuels (RSF)", "lang": "en"}, {"value": "Erneuerbare Sekundärbrennstoffe (RSF)", "lang": "de"}], "type": "flow data set", "refObjectId": "64333088-a55f-4aa2-9a31-c10b07816787", "uri": "../flows/64333088-a55f-4aa2-9a31-c10b07816787.xml"}, "exchange direction": "INPUT", "other": {"anies": [{"name": "referenceToUnitGroupDataSet", "value": {"shortDescription": [{"value": "MJ", "lang": "en"}], "type": "unit group data set", "refObjectId": "93a60a57-a3c8-11da-a746-0800200c9a66", "uri": "../unitgroups/93a60a57-a3c8-11da-a746-0800200c9a66.xml"}}, {"value": "0", "module": "A1-A3"}, {"value": "0", "module": "A4"}, {"value": "0", "module": "A5"}, {"value": "0", "module": "B1"}, {"value": "0", "module": "B2"}, {"value": "0", "module": "C1"}, {"value": "0", "module": "C2"}, {"value": "0", "module": "C3"}, {"value": "0", "module": "C4"}, {"value": "0", "module": "D"}]}, "resolvedFlowVersion": "38.00.000", "flowProperties": [], "typeOfFlow": "Other flow", "classification": {"classHierarchy": "Quantities / Environmental quantities / EPD EN 15804 / LCI indicators", "name": "GaBiCategories"}}, {"dataSetInternalID": 9, "referenceToFlowDataSet": {"shortDescription": [{"value": "Use of non renewable secondary fuels (NRSF)", "lang": "en"}, {"value": "Nicht erneuerbare Sekundärbrennstoffe (NRSF)", "lang": "de"}], "type": "flow data set", "refObjectId": "89def144-d39a-4287-b86f-efde453ddcb2", "uri": "../flows/89def144-d39a-4287-b86f-efde453ddcb2.xml"}, "exchange direction": "INPUT", "other": {"anies": [{"name": "referenceToUnitGroupDataSet", "value": {"shortDescription": [{"value": "MJ", "lang": "en"}], "type": "unit group data set", "refObjectId": "93a60a57-a3c8-11da-a746-0800200c9a66", "uri": "../unitgroups/93a60a57-a3c8-11da-a746-0800200c9a66.xml"}}, {"value": "0", "module": "A1-A3"}, {"value": "0", "module": "A4"}, {"value": "0", "module": "A5"}, {"value": "0", "module": "B1"}, {"value": "0", "module": "B2"}, {"value": "0", "module": "C1"}, {"value": "0", "module": "C2"}, {"value": "0", "module": "C3"}, {"value": "0", "module": "C4"}, {"value": "0", "module": "D"}]}, "resolvedFlowVersion": "38.00.000", "flowProperties": [], "typeOfFlow": "Other flow", "classification": {"classHierarchy": "Quantities / Environmental quantities / EPD EN 15804 / LCI indicators", "name": "GaBiCategories"}}, {"dataSetInternalID": 10, "referenceToFlowDataSet": {"shortDescription": [{"value": "Use of net fresh water (FW)", "lang": "en"}, {"value": "Einsatz von Süßwasserressourcen (FW)", "lang": "de"}], "type": "flow data set", "refObjectId": "3cf952c8-f3a4-461d-8c96-96456ca62246", "uri": "../flows/3cf952c8-f3a4-461d-8c96-96456ca62246.xml"}, "exchange direction": "INPUT", "other": {"anies": [{"name": "referenceToUnitGroupDataSet", "value": {"shortDescription": [{"value": "m^3", "lang": "en"}], "type": "unit group data set", "refObjectId": "cd950537-0a98-4044-9ba7-9f9a68d0a504", "uri": "../unitgroups/cd950537-0a98-4044-9ba7-9f9a68d0a504.xml"}}, {"value": "0.0236284246046507", "module": "A1-A3"}, {"value": "0.000209543735773414", "module": "A4"}, {"value": "0.00931592620534353", "module": "A5"}, {"value": "0", "module": "B1"}, {"value": "0.00220197560638915", "module": "B2"}, {"value": "0", "module": "C1"}, {"value": "4.51742073961691E-05", "module": "C2"}, {"value": "0", "module": "C3"}, {"value": "5.07225097007728E-05", "module": "C4"}, {"value": "-0.000105460021245168", "module": "D"}]}, "resolvedFlowVersion": "38.00.000", "flowProperties": [], "typeOfFlow": "Other flow", "classification": {"classHierarchy": "Quantities / Environmental quantities / EPD EN 15804 / LCI indicators", "name": "GaBiCategories"}}, {"dataSetInternalID": 11, "referenceToFlowDataSet": {"shortDescription": [{"value": "Hazardous waste disposed (HWD)", "lang": "en"}, {"value": "Gefährlicher Abfall zur Deponie (HWD)", "lang": "de"}], "type": "flow data set", "refObjectId": "430f9e0f-59b2-46a0-8e0d-55e0e84948fc", "uri": "../flows/430f9e0f-59b2-46a0-8e0d-55e0e84948fc.xml"}, "exchange direction": "OUTPUT", "other": {"anies": [{"name": "referenceToUnitGroupDataSet", "value": {"shortDescription": [{"value": "kg", "lang": "en"}], "type": "unit group data set", "refObjectId": "ad38d542-3fe9-439d-9b95-2f5f7752acaf", "uri": "../unitgroups/ad38d542-3fe9-439d-9b95-2f5f7752acaf.xml"}}, {"value": "3.92056508360499E-07", "module": "A1-A3"}, {"value": "1.56448363956946E-11", "module": "A4"}, {"value": "2.3071782871454E-08", "module": "A5"}, {"value": "0", "module": "B1"}, {"value": "3.59481699537557E-10", "module": "B2"}, {"value": "0", "module": "C1"}, {"value": "3.37277123274383E-12", "module": "C2"}, {"value": "0", "module": "C3"}, {"value": "6.04425922193184E-10", "module": "C4"}, {"value": "-4.49216606550761E-11", "module": "D"}]}, "resolvedFlowVersion": "38.00.000", "flowProperties": [], "typeOfFlow": "Other flow", "classification": {"classHierarchy": "Quantities / Environmental quantities / EPD EN 15804 / LCI indicators", "name": "GaBiCategories"}}, {"dataSetInternalID": 12, "referenceToFlowDataSet": {"shortDescription": [{"value": "Non hazardous waste disposed (NHWD)", "lang": "en"}, {"value": "Entsorgter nicht gefährlicher Abfall (NHWD)", "lang": "de"}], "type": "flow data set", "refObjectId": "b29ef66b-e286-4afa-949f-62f1a7b4d7fa", "uri": "../flows/b29ef66b-e286-4afa-949f-62f1a7b4d7fa.xml"}, "exchange direction": "OUTPUT", "other": {"anies": [{"name": "referenceToUnitGroupDataSet", "value": {"shortDescription": [{"value": "kg", "lang": "en"}], "type": "unit group data set", "refObjectId": "ad38d542-3fe9-439d-9b95-2f5f7752acaf", "uri": "../unitgroups/ad38d542-3fe9-439d-9b95-2f5f7752acaf.xml"}}, {"value": "0.294092638962004", "module": "A1-A3"}, {"value": "0.000468207008706277", "module": "A4"}, {"value": "0.248398589320713", "module": "A5"}, {"value": "0", "module": "B1"}, {"value": "0.00381778497568481", "module": "B2"}, {"value": "0", "module": "C1"}, {"value": "0.000100937784837951", "module": "C2"}, {"value": "0", "module": "C3"}, {"value": "3.8808937927507", "module": "C4"}, {"value": "-0.000200579508063292", "module": "D"}]}, "resolvedFlowVersion": "38.00.000", "flowProperties": [], "typeOfFlow": "Other flow", "classification": {"classHierarchy": "Quantities / Environmental quantities / EPD EN 15804 / LCI indicators", "name": "GaBiCategories"}}, {"dataSetInternalID": 13, "referenceToFlowDataSet": {"shortDescription": [{"value": "Radioactive waste disposed (RWD)", "lang": "en"}, {"value": "Entsorgter radioaktiver Abfall (RWD)", "lang": "de"}], "type": "flow data set", "refObjectId": "3449546e-52ad-4b39-b809-9fb77cea8ff6", "uri": "../flows/3449546e-52ad-4b39-b809-9fb77cea8ff6.xml"}, "exchange direction": "OUTPUT", "other": {"anies": [{"name": "referenceToUnitGroupDataSet", "value": {"shortDescription": [{"value": "kg", "lang": "en"}], "type": "unit group data set", "refObjectId": "ad38d542-3fe9-439d-9b95-2f5f7752acaf", "uri": "../unitgroups/ad38d542-3fe9-439d-9b95-2f5f7752acaf.xml"}}, {"value": "0.00351887705874506", "module": "A1-A3"}, {"value": "4.0238708682665E-06", "module": "A4"}, {"value": "0.000204900545916478", "module": "A5"}, {"value": "0", "module": "B1"}, {"value": "0.000663799071865348", "module": "B2"}, {"value": "0", "module": "C1"}, {"value": "8.67480845788836E-07", "module": "C2"}, {"value": "0", "module": "C3"}, {"value": "4.8146704128713E-05", "module": "C4"}, {"value": "-2.33087564895574E-05", "module": "D"}]}, "resolvedFlowVersion": "38.00.000", "flowProperties": [], "typeOfFlow": "Other flow", "classification": {"classHierarchy": "Quantities / Environmental quantities / EPD EN 15804 / LCI indicators", "name": "GaBiCategories"}}, {"dataSetInternalID": 14, "referenceToFlowDataSet": {"shortDescription": [{"value": "Components for re-use (CRU)", "lang": "en"}, {"value": "Komponenten für die Wiederverwendung (CRU)", "lang": "de"}], "type": "flow data set", "refObjectId": "a2b32f97-3fc7-4af2-b209-525bc6426f33", "uri": "../flows/a2b32f97-3fc7-4af2-b209-525bc6426f33.xml"}, "exchange direction": "OUTPUT", "other": {"anies": [{"name": "referenceToUnitGroupDataSet", "value": {"shortDescription": [{"value": "kg", "lang": "en"}], "type": "unit group data set", "refObjectId": "ad38d542-3fe9-439d-9b95-2f5f7752acaf", "uri": "../unitgroups/ad38d542-3fe9-439d-9b95-2f5f7752acaf.xml"}}, {"value": "0", "module": "A1-A3"}, {"value": "0", "module": "A4"}, {"value": "0", "module": "A5"}, {"value": "0", "module": "B1"}, {"value": "0", "module": "B2"}, {"value": "0", "module": "C1"}, {"value": "0", "module": "C2"}, {"value": "0", "module": "C3"}, {"value": "0", "module": "C4"}, {"value": "0", "module": "D"}]}, "resolvedFlowVersion": "38.00.000", "flowProperties": [], "typeOfFlow": "Other flow", "classification": {"classHierarchy": "Quantities / Environmental quantities / EPD EN 15804 / LCI indicators", "name": "GaBiCategories"}}, {"dataSetInternalID": 15, "referenceToFlowDataSet": {"shortDescription": [{"value": "Materials for recycling (MFR)", "lang": "en"}, {"value": "Stoffe zum Recycling (MFR)", "lang": "de"}], "type": "flow data set", "refObjectId": "d7fe48a5-4103-49c8-9aae-b0b5dfdbd6ae", "uri": "../flows/d7fe48a5-4103-49c8-9aae-b0b5dfdbd6ae.xml"}, "exchange direction": "OUTPUT", "other": {"anies": [{"name": "referenceToUnitGroupDataSet", "value": {"shortDescription": [{"value": "kg", "lang": "en"}], "type": "unit group data set", "refObjectId": "ad38d542-3fe9-439d-9b95-2f5f7752acaf", "uri": "../unitgroups/ad38d542-3fe9-439d-9b95-2f5f7752acaf.xml"}}, {"value": "0", "module": "A1-A3"}, {"value": "0", "module": "A4"}, {"value": "0.1809136631583", "module": "A5"}, {"value": "0", "module": "B1"}, {"value": "0", "module": "B2"}, {"value": "0", "module": "C1"}, {"value": "0", "module": "C2"}, {"value": "0", "module": "C3"}, {"value": "0", "module": "C4"}, {"value": "0", "module": "D"}]}, "resolvedFlowVersion": "38.00.000", "flowProperties": [], "typeOfFlow": "Other flow", "classification": {"classHierarchy": "Quantities / Environmental quantities / EPD EN 15804 / LCI indicators", "name": "GaBiCategories"}}, {"dataSetInternalID": 16, "referenceToFlowDataSet": {"shortDescription": [{"value": "Materials for energy recovery (MER)", "lang": "en"}, {"value": "Stoffe für die Energierückgewinnung (MER)", "lang": "de"}], "type": "flow data set", "refObjectId": "59a9181c-3aaf-46ee-8b13-2b3723b6e447", "uri": "../flows/59a9181c-3aaf-46ee-8b13-2b3723b6e447.xml"}, "exchange direction": "OUTPUT", "other": {"anies": [{"name": "referenceToUnitGroupDataSet", "value": {"shortDescription": [{"value": "kg", "lang": "en"}], "type": "unit group data set", "refObjectId": "ad38d542-3fe9-439d-9b95-2f5f7752acaf", "uri": "../unitgroups/ad38d542-3fe9-439d-9b95-2f5f7752acaf.xml"}}, {"value": "0", "module": "A1-A3"}, {"value": "0", "module": "A4"}, {"value": "0", "module": "A5"}, {"value": "0", "module": "B1"}, {"value": "0", "module": "B2"}, {"value": "0", "module": "C1"}, {"value": "0", "module": "C2"}, {"value": "0", "module": "C3"}, {"value": "0", "module": "C4"}, {"value": "0", "module": "D"}]}, "resolvedFlowVersion": "38.00.000", "flowProperties": [], "typeOfFlow": "Other flow", "classification": {"classHierarchy": "Quantities / Environmental quantities / EPD EN 15804 / LCI indicators", "name": "GaBiCategories"}}, {"dataSetInternalID": 17, "referenceToFlowDataSet": {"shortDescription": [{"value": "Exported electrical energy (EEE)", "lang": "en"}, {"value": "Exportierte elektrische Energie (EEE)", "lang": "de"}], "type": "flow data set", "refObjectId": "4da0c987-2b76-40d6-9e9e-82a017aaaf29", "uri": "../flows/4da0c987-2b76-40d6-9e9e-82a017aaaf29.xml"}, "exchange direction": "OUTPUT", "other": {"anies": [{"name": "referenceToUnitGroupDataSet", "value": {"shortDescription": [{"value": "MJ", "lang": "en"}], "type": "unit group data set", "refObjectId": "93a60a57-a3c8-11da-a746-0800200c9a66", "uri": "../unitgroups/93a60a57-a3c8-11da-a746-0800200c9a66.xml"}}, {"value": "0", "module": "A1-A3"}, {"value": "0", "module": "A4"}, {"value": "0.0636508991090628", "module": "A5"}, {"value": "0", "module": "B1"}, {"value": "0", "module": "B2"}, {"value": "0", "module": "C1"}, {"value": "0", "module": "C2"}, {"value": "0", "module": "C3"}, {"value": "0", "module": "C4"}, {"value": "0", "module": "D"}]}, "resolvedFlowVersion": "38.00.000", "flowProperties": [], "typeOfFlow": "Other flow", "classification": {"classHierarchy": "Quantities / Environmental quantities / EPD EN 15804 / LCI indicators", "name": "GaBiCategories"}}, {"dataSetInternalID": 18, "referenceToFlowDataSet": {"shortDescription": [{"value": "Exported thermal energy (EET)", "lang": "en"}, {"value": "Exportierte thermische Energie (EET)", "lang": "de"}], "type": "flow data set", "refObjectId": "98daf38a-7a79-46d3-9a37-2b7bd0955810", "uri": "../flows/98daf38a-7a79-46d3-9a37-2b7bd0955810.xml"}, "exchange direction": "OUTPUT", "other": {"anies": [{"name": "referenceToUnitGroupDataSet", "value": {"shortDescription": [{"value": "MJ", "lang": "en"}], "type": "unit group data set", "refObjectId": "93a60a57-a3c8-11da-a746-0800200c9a66", "uri": "../unitgroups/93a60a57-a3c8-11da-a746-0800200c9a66.xml"}}, {"value": "0", "module": "A1-A3"}, {"value": "0", "module": "A4"}, {"value": "0.0976949264004297", "module": "A5"}, {"value": "0", "module": "B1"}, {"value": "0", "module": "B2"}, {"value": "0", "module": "C1"}, {"value": "0", "module": "C2"}, {"value": "0", "module": "C3"}, {"value": "0", "module": "C4"}, {"value": "0", "module": "D"}]}, "resolvedFlowVersion": "38.00.000", "flowProperties": [], "typeOfFlow": "Other flow", "classification": {"classHierarchy": "Quantities / Environmental quantities / EPD EN 15804 / LCI indicators", "name": "GaBiCategories"}}]}, "LCIAResults": {"LCIAResult": [{"referenceToLCIAMethodDataSet": {"shortDescription": [{"value": "Global Warming Potential total (GWP-total)", "lang": "en"}, {"value": "Globales Erwärmungspotenzial total (GWP-total)", "lang": "de"}], "type": "LCIA method data set", "refObjectId": "6a37f984-a4b3-458a-a20a-64418c145fa2", "uri": "../lciamethods/6a37f984-a4b3-458a-a20a-64418c145fa2.xml"}, "other": {"anies": [{"name": "referenceToUnitGroupDataSet", "value": {"shortDescription": [{"value": "kg CO_(2) eq", "lang": "en"}], "type": "unit group data set", "refObjectId": "1ebf3012-d0db-4de2-aefd-ef30cedb0be1", "uri": "../unitgroups/1ebf3012-d0db-4de2-aefd-ef30cedb0be1.xml"}}, {"value": "7.57896128386982", "module": "A1-A3"}, {"value": "0.244826966746924", "module": "A4"}, {"value": "0.504859190679898", "module": "A5"}, {"value": "0.000253855975702815", "module": "B1"}, {"value": "0.23159830205469", "module": "B2"}, {"value": "0", "module": "C1"}, {"value": "0.0527806957873457", "module": "C2"}, {"value": "0", "module": "C3"}, {"value": "0.273348963523101", "module": "C4"}, {"value": "-0.0172359359626743", "module": "D"}]}}, {"referenceToLCIAMethodDataSet": {"shortDescription": [{"value": "Global Warming Potential fossil fuels (GWP-fossil)", "lang": "en"}, {"value": "Globales Erwärmungspotenzial fossil (GWP-fossil)", "lang": "de"}], "type": "LCIA method data set", "refObjectId": "5f635281-343e-44fb-83df-1971b155e6b6", "uri": "../lciamethods/5f635281-343e-44fb-83df-1971b155e6b6.xml"}, "other": {"anies": [{"name": "referenceToUnitGroupDataSet", "value": {"shortDescription": [{"value": "kg CO_(2) eq", "lang": "en"}], "type": "unit group data set", "refObjectId": "1ebf3012-d0db-4de2-aefd-ef30cedb0be1", "uri": "../unitgroups/1ebf3012-d0db-4de2-aefd-ef30cedb0be1.xml"}}, {"value": "7.90329216598311", "module": "A1-A3"}, {"value": "0.243804098841174", "module": "A4"}, {"value": "0.508209445528591", "module": "A5"}, {"value": "0.000253855975702815", "module": "B1"}, {"value": "0.229107803534055", "module": "B2"}, {"value": "0", "module": "C1"}, {"value": "0.0525601821712136", "module": "C2"}, {"value": "0", "module": "C3"}, {"value": "0.276153620765658", "module": "C4"}, {"value": "-0.0211095964859132", "module": "D"}]}}, {"referenceToLCIAMethodDataSet": {"shortDescription": [{"value": "Global Warming Potential biogenic (GWP-biogenic)", "lang": "en"}, {"value": "Globales Erwärmungspotenzial biogen (GWP-biogenic)", "lang": "de"}], "type": "LCIA method data set", "refObjectId": "2356e1ab-0185-4db5-86e5-16de51c7485c", "uri": "../lciamethods/2356e1ab-0185-4db5-86e5-16de51c7485c.xml"}, "other": {"anies": [{"name": "referenceToUnitGroupDataSet", "value": {"shortDescription": [{"value": "kg CO_(2) eq", "lang": "en"}], "type": "unit group data set", "refObjectId": "1ebf3012-d0db-4de2-aefd-ef30cedb0be1", "uri": "../unitgroups/1ebf3012-d0db-4de2-aefd-ef30cedb0be1.xml"}}, {"value": "-0.327713956255358", "module": "A1-A3"}, {"value": "-0.00033685886133587", "module": "A4"}, {"value": "-0.00363774292059373", "module": "A5"}, {"value": "0", "module": "B1"}, {"value": "0.00244204161172588", "module": "B2"}, {"value": "0", "module": "C1"}, {"value": "-7.26212692975883E-05", "module": "C2"}, {"value": "0", "module": "C3"}, {"value": "-0.00293909940279343", "module": "C4"}, {"value": "0.00387684646060226", "module": "D"}]}}, {"referenceToLCIAMethodDataSet": {"shortDescription": [{"value": "Global Warming Potential luluc (GWP-luluc)", "lang": "en"}, {"value": "Globales Erwärmungspotenzial luluc (GWP-luluc)", "lang": "de"}], "type": "LCIA method data set", "refObjectId": "4331bbdb-978a-490d-8707-eeb047f01a55", "uri": "../lciamethods/4331bbdb-978a-490d-8707-eeb047f01a55.xml"}, "other": {"anies": [{"name": "referenceToUnitGroupDataSet", "value": {"shortDescription": [{"value": "kg CO_(2) eq", "lang": "en"}], "type": "unit group data set", "refObjectId": "1ebf3012-d0db-4de2-aefd-ef30cedb0be1", "uri": "../unitgroups/1ebf3012-d0db-4de2-aefd-ef30cedb0be1.xml"}}, {"value": "0.00338307414206639", "module": "A1-A3"}, {"value": "0.00135972676708568", "module": "A4"}, {"value": "0.000287488071900762", "module": "A5"}, {"value": "0", "module": "B1"}, {"value": "4.84569089094039E-05", "module": "B2"}, {"value": "0", "module": "C1"}, {"value": "0.000293134885429699", "module": "C2"}, {"value": "0", "module": "C3"}, {"value": "0.00013444216023718", "module": "C4"}, {"value": "-3.1859373633021E-06", "module": "D"}]}}, {"referenceToLCIAMethodDataSet": {"shortDescription": [{"value": "Depletion potential of the stratospheric ozone layer (ODP)", "lang": "en"}, {"value": "Abbau Potential der stratosphärischen Ozonschicht (ODP)", "lang": "de"}], "type": "LCIA method data set", "refObjectId": "b5c629d6-def3-11e6-bf01-fe55135034f3", "uri": "../lciamethods/b5c629d6-def3-11e6-bf01-fe55135034f3.xml"}, "other": {"anies": [{"name": "referenceToUnitGroupDataSet", "value": {"shortDescription": [{"value": "kg CFC11 eq", "lang": "en"}], "type": "unit group data set", "refObjectId": "d9e957c9-7309-4474-bf3a-7777df6c4e5b", "uri": "../unitgroups/d9e957c9-7309-4474-bf3a-7777df6c4e5b.xml"}}, {"value": "8.28441361989349E-09", "module": "A1-A3"}, {"value": "1.4611709794452E-14", "module": "A4"}, {"value": "4.36250642297673E-10", "module": "A5"}, {"value": "0", "module": "B1"}, {"value": "3.35031408002072E-12", "module": "B2"}, {"value": "0", "module": "C1"}, {"value": "3.15004600939711E-15", "module": "C2"}, {"value": "0", "module": "C3"}, {"value": "3.70929023746361E-13", "module": "C4"}, {"value": "-1.21509992347486E-13", "module": "D"}]}}, {"referenceToLCIAMethodDataSet": {"shortDescription": [{"value": "Acidification potential of land and water (AP)", "lang": "en"}, {"value": "Versauerungspotenzial von Boden und Wasser (AP)", "lang": "de"}], "type": "LCIA method data set", "refObjectId": "b5c611c6-def3-11e6-bf01-fe55135034f3", "uri": "../lciamethods/b5c611c6-def3-11e6-bf01-fe55135034f3.xml"}, "other": {"anies": [{"name": "referenceToUnitGroupDataSet", "value": {"shortDescription": [{"value": "mol H^(+) eq", "lang": "en"}], "type": "unit group data set", "refObjectId": "42e089ac-92bf-4bf2-8ca1-5fc40d18f2ed", "uri": "../unitgroups/42e089ac-92bf-4bf2-8ca1-5fc40d18f2ed.xml"}}, {"value": "0.0143354783334266", "module": "A1-A3"}, {"value": "0.000251289461062306", "module": "A4"}, {"value": "0.00116890311417556", "module": "A5"}, {"value": "0", "module": "B1"}, {"value": "0.000502972932487876", "module": "B2"}, {"value": "0", "module": "C1"}, {"value": "5.41739040234311E-05", "module": "C2"}, {"value": "0", "module": "C3"}, {"value": "0.000818450613024772", "module": "C4"}, {"value": "-3.46847385724995E-05", "module": "D"}]}}, {"referenceToLCIAMethodDataSet": {"shortDescription": [{"value": "Eutrophication potential aquatic freshwater (EP-freshwater)", "lang": "en"}, {"value": "Eutrophierungspotenzial Süßwasser (EP-freshwater)", "lang": "de"}], "type": "LCIA method data set", "refObjectId": "b53ec18f-7377-4ad3-86eb-cc3f4f276b2b", "uri": "../lciamethods/b53ec18f-7377-4ad3-86eb-cc3f4f276b2b.xml"}, "other": {"anies": [{"name": "referenceToUnitGroupDataSet", "value": {"shortDescription": [{"value": "kg P eq", "lang": "en"}], "type": "unit group data set", "refObjectId": "0429039d-a61d-4590-ba67-aa4a20a810a1", "uri": "../unitgroups/0429039d-a61d-4590-ba67-aa4a20a810a1.xml"}}, {"value": "2.06601558314979E-05", "module": "A1-A3"}, {"value": "7.27990055691823E-07", "module": "A4"}, {"value": "1.57232718734335E-05", "module": "A5"}, {"value": "0", "module": "B1"}, {"value": "1.11829299188137E-06", "module": "B2"}, {"value": "0", "module": "C1"}, {"value": "1.56942767278579E-07", "module": "C2"}, {"value": "0", "module": "C3"}, {"value": "5.15498604248783E-05", "module": "C4"}, {"value": "-3.07928853890359E-08", "module": "D"}]}}, {"referenceToLCIAMethodDataSet": {"shortDescription": [{"value": "Eutrophication potential aquatic marine (EP-marine)", "lang": "en"}, {"value": "Eutrophierungspotenzial Salzwasser (EP-marine)", "lang": "de"}], "type": "LCIA method data set", "refObjectId": "b5c619fa-def3-11e6-bf01-fe55135034f3", "uri": "../lciamethods/b5c619fa-def3-11e6-bf01-fe55135034f3.xml"}, "other": {"anies": [{"name": "referenceToUnitGroupDataSet", "value": {"shortDescription": [{"value": "kg N eq", "lang": "en"}], "type": "unit group data set", "refObjectId": "d05bb823-ecdf-4686-8c40-bf1d9257859f", "uri": "../unitgroups/d05bb823-ecdf-4686-8c40-bf1d9257859f.xml"}}, {"value": "0.00363282091566006", "module": "A1-A3"}, {"value": "8.22118534453409E-05", "module": "A4"}, {"value": "0.000265856403852531", "module": "A5"}, {"value": "0", "module": "B1"}, {"value": "0.000114597600645661", "module": "B2"}, {"value": "0", "module": "C1"}, {"value": "1.7723533009735E-05", "module": "C2"}, {"value": "0", "module": "C3"}, {"value": "0.000181071453348141", "module": "C4"}, {"value": "-9.64073280011374E-06", "module": "D"}]}}, {"referenceToLCIAMethodDataSet": {"shortDescription": [{"value": "Eutrophication potential terrestrial (EP-terrestrial)", "lang": "en"}, {"value": "Eutrophierungspotenzial Land (EP-terrestrial)", "lang": "de"}], "type": "LCIA method data set", "refObjectId": "b5c614d2-def3-11e6-bf01-fe55135034f3", "uri": "../lciamethods/b5c614d2-def3-11e6-bf01-fe55135034f3.xml"}, "other": {"anies": [{"name": "referenceToUnitGroupDataSet", "value": {"shortDescription": [{"value": "mol N eq", "lang": "en"}], "type": "unit group data set", "refObjectId": "71b4d617-0ec9-4d3f-b65e-e438940c2401", "uri": "../unitgroups/71b4d617-0ec9-4d3f-b65e-e438940c2401.xml"}}, {"value": "0.0345981075549234", "module": "A1-A3"}, {"value": "0.000978609330522475", "module": "A4"}, {"value": "0.00327407145862402", "module": "A5"}, {"value": "0", "module": "B1"}, {"value": "0.00118462981204945", "module": "B2"}, {"value": "0", "module": "C1"}, {"value": "0.000210972190095206", "module": "C2"}, {"value": "0", "module": "C3"}, {"value": "0.0019859204425069", "module": "C4"}, {"value": "-0.000103303403670862", "module": "D"}]}}, {"referenceToLCIAMethodDataSet": {"shortDescription": [{"value": "Formation potential of tropospheric ozone photochemical oxidants (POCP)", "lang": "en"}, {"value": "Bildungspotential für troposphärisches Ozon (POCP)", "lang": "de"}], "type": "LCIA method data set", "refObjectId": "b5c610fe-def3-11e6-bf01-fe55135034f3", "uri": "../lciamethods/b5c610fe-def3-11e6-bf01-fe55135034f3.xml"}, "other": {"anies": [{"name": "referenceToUnitGroupDataSet", "value": {"shortDescription": [{"value": "kg NMVOC eq", "lang": "en"}], "type": "unit group data set", "refObjectId": "d27c25f8-fbc1-44c6-b47b-4adbae4199c6", "uri": "../unitgroups/d27c25f8-fbc1-44c6-b47b-4adbae4199c6.xml"}}, {"value": "0.012152354779732", "module": "A1-A3"}, {"value": "0.000221397637495026", "module": "A4"}, {"value": "0.000972445306404923", "module": "A5"}, {"value": "1.41031097612675E-05", "module": "B1"}, {"value": "0.000305201574250449", "module": "B2"}, {"value": "0", "module": "C1"}, {"value": "4.77297150225336E-05", "module": "C2"}, {"value": "0", "module": "C3"}, {"value": "0.000582502725472966", "module": "C4"}, {"value": "-3.14428110678558E-05", "module": "D"}]}}, {"referenceToLCIAMethodDataSet": {"shortDescription": [{"value": "Abiotic depletion potential for non fossil resources (ADPE)", "lang": "en"}, {"value": "Potenzial für den abiotischen Abbau nicht fossiler Ressourcen (ADPE)", "lang": "de"}], "type": "LCIA method data set", "refObjectId": "b2ad6494-c78d-11e6-9d9d-cec0c932ce01", "uri": "../lciamethods/b2ad6494-c78d-11e6-9d9d-cec0c932ce01.xml"}, "other": {"anies": [{"name": "referenceToUnitGroupDataSet", "value": {"shortDescription": [{"value": "kg Sb eq", "lang": "en"}], "type": "unit group data set", "refObjectId": "54ccd2d9-a32a-4fc2-923d-f2c8c93e89d4", "uri": "../unitgroups/54ccd2d9-a32a-4fc2-923d-f2c8c93e89d4.xml"}}, {"value": "1.03518768649931E-06", "module": "A1-A3"}, {"value": "2.03882169291753E-08", "module": "A4"}, {"value": "7.98585549482882E-08", "module": "A5"}, {"value": "0", "module": "B1"}, {"value": "6.23687996348645E-08", "module": "B2"}, {"value": "0", "module": "C1"}, {"value": "4.39536661211662E-09", "module": "C2"}, {"value": "0", "module": "C3"}, {"value": "1.91509646976157E-08", "module": "C4"}, {"value": "-3.33268904281349E-09", "module": "D"}]}}, {"referenceToLCIAMethodDataSet": {"shortDescription": [{"value": "Abiotic depletion potential for fossil resources (ADPF)", "lang": "en"}, {"value": "Potenzial für den abiotischen Abbau fossiler Brennstoffe (ADPF)", "lang": "de"}], "type": "LCIA method data set", "refObjectId": "b2ad6110-c78d-11e6-9d9d-cec0c932ce01", "uri": "../lciamethods/b2ad6110-c78d-11e6-9d9d-cec0c932ce01.xml"}, "other": {"anies": [{"name": "referenceToUnitGroupDataSet", "value": {"shortDescription": [{"value": "MJ", "lang": "en"}], "type": "unit group data set", "refObjectId": "93a60a57-a3c8-11da-a746-0800200c9a66", "uri": "../unitgroups/93a60a57-a3c8-11da-a746-0800200c9a66.xml"}}, {"value": "173.004541538497", "module": "A1-A3"}, {"value": "3.25919641273985", "module": "A4"}, {"value": "10.4937480316712", "module": "A5"}, {"value": "0", "module": "B1"}, {"value": "4.15336944363877", "module": "B2"}, {"value": "0", "module": "C1"}, {"value": "0.702629520994922", "module": "C2"}, {"value": "0", "module": "C3"}, {"value": "3.91876279629675", "module": "C4"}, {"value": "-0.501472199887886", "module": "D"}]}}, {"referenceToLCIAMethodDataSet": {"shortDescription": [{"value": "Water use (WDP)", "lang": "en"}, {"value": "Wassernutzung (WDP)", "lang": "de"}], "type": "LCIA method data set", "refObjectId": "b2ad66ce-c78d-11e6-9d9d-cec0c932ce01", "uri": "../lciamethods/b2ad66ce-c78d-11e6-9d9d-cec0c932ce01.xml"}, "other": {"anies": [{"name": "referenceToUnitGroupDataSet", "value": {"shortDescription": [{"value": "m^(3) world eq deprived", "lang": "en"}], "type": "unit group data set", "refObjectId": "6ae2df01-888e-46c8-b17d-49fa3869b476", "uri": "../unitgroups/6ae2df01-888e-46c8-b17d-49fa3869b476.xml"}}, {"value": "0.357301523265804", "module": "A1-A3"}, {"value": "0.00218762795429583", "module": "A4"}, {"value": "0.0886243660387661", "module": "A5"}, {"value": "0", "module": "B1"}, {"value": "0.0523130615294909", "module": "B2"}, {"value": "0", "module": "C1"}, {"value": "0.000471616861025513", "module": "C2"}, {"value": "0", "module": "C3"}, {"value": "-0.00272257567773984", "module": "C4"}, {"value": "-0.00298252933294688", "module": "D"}]}}, {"referenceToLCIAMethodDataSet": {"shortDescription": [{"value": "Incidence of disease due to PM emissions (PM)", "lang": "en"}, {"value": "Auftreten von Krankheiten aufgrund von Feinstaubemissionen (PM)", "lang": "de"}], "type": "LCIA method data set", "refObjectId": "b5c602c6-def3-11e6-bf01-fe55135034f3", "uri": "../lciamethods/b5c602c6-def3-11e6-bf01-fe55135034f3.xml"}, "other": {"anies": [{"name": "referenceToUnitGroupDataSet", "value": {"shortDescription": [{"value": "Disease incidence", "lang": "en"}], "type": "unit group data set", "refObjectId": "3883559b-648f-4afc-8ba2-0bd24f3affa3", "uri": "../unitgroups/3883559b-648f-4afc-8ba2-0bd24f3affa3.xml"}}, {"value": "1.36145725341397E-07", "module": "A1-A3"}, {"value": "1.45076017090295E-09", "module": "A4"}, {"value": "1.2018823088857E-08", "module": "A5"}, {"value": "0", "module": "B1"}, {"value": "4.17185802808898E-09", "module": "B2"}, {"value": "0", "module": "C1"}, {"value": "3.12760200635817E-10", "module": "C2"}, {"value": "0", "module": "C3"}, {"value": "7.86573524307626E-09", "module": "C4"}, {"value": "-7.86733772251991E-10", "module": "D"}]}}, {"referenceToLCIAMethodDataSet": {"shortDescription": [{"value": "Human exposure efficiency relative to U235 (IR)", "lang": "en"}, {"value": "Wirkung durch Exposition des Menschen mit U235 (IR)", "lang": "de"}], "type": "LCIA method data set", "refObjectId": "b5c632be-def3-11e6-bf01-fe55135034f3", "uri": "../lciamethods/b5c632be-def3-11e6-bf01-fe55135034f3.xml"}, "other": {"anies": [{"name": "referenceToUnitGroupDataSet", "value": {"shortDescription": [{"value": "kBq U235 eq", "lang": "en"}], "type": "unit group data set", "refObjectId": "456b05bf-1415-44a9-9993-02452f554c09", "uri": "../unitgroups/456b05bf-1415-44a9-9993-02452f554c09.xml"}}, {"value": "0.37585429538253", "module": "A1-A3"}, {"value": "0.000589661920829667", "module": "A4"}, {"value": "0.0223533048680777", "module": "A5"}, {"value": "0", "module": "B1"}, {"value": "0.112450126215392", "module": "B2"}, {"value": "0", "module": "C1"}, {"value": "0.000127121480424434", "module": "C2"}, {"value": "0", "module": "C3"}, {"value": "0.00710726215781642", "module": "C4"}, {"value": "-0.00392187658063854", "module": "D"}]}}, {"referenceToLCIAMethodDataSet": {"shortDescription": [{"value": "Comparative toxic unit for ecosystems (ETP-fw)", "lang": "en"}, {"value": "Toxizitätsvergleichseinheit für Ökosysteme (ETP-fw)", "lang": "de"}], "type": "LCIA method data set", "refObjectId": "ee1082d1-b0f7-43ca-a1f0-21e2a4a74511", "uri": "../lciamethods/ee1082d1-b0f7-43ca-a1f0-21e2a4a74511.xml"}, "other": {"anies": [{"name": "referenceToUnitGroupDataSet", "value": {"shortDescription": [{"value": "CTUe", "lang": "en"}], "type": "unit group data set", "refObjectId": "aa959ded-f1eb-4efb-9c5c-2d60be36b3e6", "uri": "../unitgroups/aa959ded-f1eb-4efb-9c5c-2d60be36b3e6.xml"}}, {"value": "92.8287559459512", "module": "A1-A3"}, {"value": "2.26270939704295", "module": "A4"}, {"value": "5.93182295500623", "module": "A5"}, {"value": "0.000115063371682035", "module": "B1"}, {"value": "1.87846564490847", "module": "B2"}, {"value": "0", "module": "C1"}, {"value": "0.487803193934694", "module": "C2"}, {"value": "0", "module": "C3"}, {"value": "3.83487626083584", "module": "C4"}, {"value": "-0.194162794120119", "module": "D"}]}}, {"referenceToLCIAMethodDataSet": {"shortDescription": [{"value": "Comparative toxic unit for humans (carcinogenic) (HTP-c)", "lang": "en"}, {"value": "Toxizitätsvergleichseinheit für Menschen (krebserregend) (HTP-c)", "lang": "de"}], "type": "LCIA method data set", "refObjectId": "2299222a-bbd8-474f-9d4f-4dd1f18aea7c", "uri": "../lciamethods/2299222a-bbd8-474f-9d4f-4dd1f18aea7c.xml"}, "other": {"anies": [{"name": "referenceToUnitGroupDataSet", "value": {"shortDescription": [{"value": "CTUh", "lang": "en"}], "type": "unit group data set", "refObjectId": "d4c9523e-2d7e-49fd-8469-998f547d3a70", "uri": "../unitgroups/d4c9523e-2d7e-49fd-8469-998f547d3a70.xml"}}, {"value": "2.63785894535567E-09", "module": "A1-A3"}, {"value": "4.56069951554961E-11", "module": "A4"}, {"value": "1.75703477813327E-10", "module": "A5"}, {"value": "0", "module": "B1"}, {"value": "5.42944701402369E-11", "module": "B2"}, {"value": "0", "module": "C1"}, {"value": "9.83212335251233E-12", "module": "C2"}, {"value": "0", "module": "C3"}, {"value": "1.72194285497565E-10", "module": "C4"}, {"value": "-5.74753940388982E-12", "module": "D"}]}}, {"referenceToLCIAMethodDataSet": {"shortDescription": [{"value": "Comparative toxic unit for humans (noncarcinogenic) (HTP-nc)", "lang": "en"}, {"value": "Toxizitätsvergleichseinheit für Menschen (nicht krebserregend) (HTP-nc)", "lang": "de"}], "type": "LCIA method data set", "refObjectId": "3af763a5-b7a1-48c9-9cee-1f223481fcef", "uri": "../lciamethods/3af763a5-b7a1-48c9-9cee-1f223481fcef.xml"}, "other": {"anies": [{"name": "referenceToUnitGroupDataSet", "value": {"shortDescription": [{"value": "CTUh", "lang": "en"}], "type": "unit group data set", "refObjectId": "d4c9523e-2d7e-49fd-8469-998f547d3a70", "uri": "../unitgroups/d4c9523e-2d7e-49fd-8469-998f547d3a70.xml"}}, {"value": "1.33640698928052E-07", "module": "A1-A3"}, {"value": "2.36659050975545E-09", "module": "A4"}, {"value": "9.28072181685394E-09", "module": "A5"}, {"value": "3.06571599593443E-12", "module": "B1"}, {"value": "2.1238774522098E-09", "module": "B2"}, {"value": "0", "module": "C1"}, {"value": "5.10198265364048E-10", "module": "C2"}, {"value": "0", "module": "C3"}, {"value": "1.44319669454389E-08", "module": "C4"}, {"value": "-2.23957544385625E-10", "module": "D"}]}}, {"referenceToLCIAMethodDataSet": {"shortDescription": [{"value": "Soil quality index (SQP)", "lang": "en"}, {"value": "Bodenqualitätsindex (SQP)", "lang": "de"}], "type": "LCIA method data set", "refObjectId": "b2ad6890-c78d-11e6-9d9d-cec0c932ce01", "uri": "../lciamethods/b2ad6890-c78d-11e6-9d9d-cec0c932ce01.xml"}, "other": {"anies": [{"name": "referenceToUnitGroupDataSet", "value": {"shortDescription": [{"value": "SQP", "lang": "en"}], "type": "unit group data set", "refObjectId": "f130951c-e67f-4f7f-8dd4-665de3974e18", "uri": "../unitgroups/f130951c-e67f-4f7f-8dd4-665de3974e18.xml"}}, {"value": "14.0187057907255", "module": "A1-A3"}, {"value": "1.12148420541512", "module": "A4"}, {"value": "11.1578597766437", "module": "A5"}, {"value": "0", "module": "B1"}, {"value": "1.49746469005059", "module": "B2"}, {"value": "0", "module": "C1"}, {"value": "0.241773679847596", "module": "C2"}, {"value": "0", "module": "C3"}, {"value": "0.281954195417485", "module": "C4"}, {"value": "-0.646729723954846", "module": "D"}]}}]}, "otherAttributes": {"{http://www.indata.network/EPD/2019}epd-version": "1.2"}, "version": "1.1", "locations": "../ILCDLocations.xml"}