{"processInformation": {"dataSetInformation": {"UUID": "8028fe64-1856-4000-9ee5-14550448d02f", "name": {"baseName": [{"value": "Spannbeton-Weichenschwellen, TSF-A", "lang": "de"}, {"value": "Concrete turnout sleeper, TSF-A", "lang": "en"}], "functionalUnitFlowProperties": [{"lang": "de"}]}, "classificationInformation": {"classification": [{"class": [{"value": "Mineralische Baustoffe", "level": 0, "classId": "1"}, {"value": "Mörtel und Beton", "level": 1, "classId": "1.4"}, {"value": "Beton", "level": 2, "classId": "1.4.01"}], "name": "OEKOBAU.DAT"}, {"class": [{"value": "02 Bauprodukte", "level": 0}, {"value": "Normal- Leicht- und Porenbeton", "level": 1}, {"value": "Betonfertigteile", "level": 2}], "name": "IBUCategories"}]}, "generalComment": [{"value": "Die TSF-A GmbH (Turnout Sleeper Factory-Austria) wurde 2008 als Joint Venture zwischen der Kirchdorfer Fertigteilholding GmbH und der voestalpine Turnout Technology Zeltweg GmbH gegründet. Durch die jahrzehntelange Erfahrung beider Unternehmen im jeweiligen Fachbereich - der Entwicklung und Produktion von Weichenbetonschwellen sowie der Bereitstellung kompletter Weichensystemen - können Synergien bestens genutzt und die Weichenbeton-schwellen im Gesamtsystem optimiert und weiterentwickelt werden. \n\nMit der Gründung der voestalpine Railway Systems GmbH im Jahr 2020 ist die TSF-A nun Teil des weltweit führenden Anbieters von Systemlösungen für die Bahninfrastruktur. \n\nDie TSF-A bietet verschiedene Typen hochqualitativer, vorgespannter Weichenbetonschwellen, wahlweise mit Besohlung und vormontierten Befestigungssystemen an.\n\nBei den deklarierten Produkten handelt es sich um vorgespannte Fertigteile aus Beton in unterschiedlichen Größen und Ausführungen zur Verwendung als Weichenbetonschwellen. Weichenbetonschwellen stützen und halten die Schienen und Weichenkomponenten in der richtigen Position und übertragen die Lasten auf den Bahnoberbau.\n\nDer Spannbeton wird aus \n\nvorgespanntem Spannstahl,\nZement (hydraulisches Bindemittel),\nSplitt und Sand unterschiedlicher Gesteinskörnungen (Zuschlagsstoffe),\nWasser und\nZusatzmitteln und Zusatzstoffen hergestellt. \n\nEinbetonierte Kunststoffteile der Dübelbefestigung bilden die Anker für die Verschraubung der Schienenbefestigungssysteme. Je nach Ausführung sind zusätzliche Bewehrungselemente wie Endbügel bzw. Dübelbewehrungen aus Stahl inkludiert.\n\nJe nach Bedarf werden die Weichenbetonschwellen besohlt oder unbesohlt, beziehungsweise mit vormontierten Rippenplatten und/oder Befestigungsmaterial geliefert. Die Grundgeometrie der Weichenschwelle kann in Höhe, Sohlenbreite und Ausführung variieren.\n\nEine mögliche Aufplattung mit Komponenten von Befestigungssystemen, wie stählerne Rippenplatten, metallische Befestigungsmittel, polymere Zwischenlagen und -platten sowie Winkelführungsplatten, erfolgt in einem separaten Arbeitsgang und wird in der vorliegenden EPD nicht berücksichtigt. \n\nDie deklarierten Produkte werden nach den gültigen europäischen und internationalen Normen, Richtlinien und div. Kundenspezifikationen gefertigt und ausgeliefert.", "lang": "de"}, {"value": "TSF-A GmbH (Turnout Sleeper Factory-Austria) was founded in 2008 as a joint venture between Kirchdorfer Fertigteilholding GmbH and voestalpine Turnout Technology Zeltweg GmbH. \n\nThanks to the decades of experience of both companies in the respective specialist area of railway infrastructure business - the development and production of concrete turnout sleepers and the provision of complete turnout systems - the concrete turnout sleepers can be optimized and further developed in the overall system.\n\nWith the founding of voestalpine Railway Systems GmbH in 2020, TSF-A is now part of the world's leading provider of system solutions for rail infrastructure.\n\nTSF-A offers different types of high quality, prestressed concrete turnout sleepers, optionally with under sleeper pads and fastening systems.\n\nThe declared products are prestressed concrete parts of different size and design for use as concrete turnout sleepers. The concrete turnout sleepers support and keep the rails and turnout components in the correct position and transfer the loads to the track superstructure.\n\n\nThe concrete consists of\n\n• prestressed steel,\n\n• cement (hydraulic binder),\n\n• sand and gravel of different grain sizes (aggregates)\n\n• water and\n\n• admixtures and additives.\n\nCast-in plastic parts of a dowel fastener form the anchor for attaching the rail fastening systems. Depending on the design of the fastening system, additional reinforcement elements such as end brackets or dowel reinforcements made of steel are required.\n\nDepending on the requirements, the concrete turnout sleepers may be alternatively supplied pre-assembled with under sleeper pads, ribbed base plates or fastening material for rails.\n\nA possible pre-assembly takes place in a separate work step within the plants and is not taken into account in this EPD.\n\nThe basic geometry of the turnout sleeper can vary in height, width and design.\n\n\nThe declared products are manufactured and delivered in accordance with the applicable European and international standards, guidelines and various customer specifications.", "lang": "en"}]}, "quantitativeReference": {"referenceToReferenceFlow": [0]}, "time": {"referenceYear": 2021, "dataSetValidUntil": 2026, "other": {"anies": [{"name": "publicationDateOfEPD", "value": 1625097600000}]}}, "geography": {"locationOfOperationSupplyOrProduction": {"location": "AT"}}, "technology": {"technologyDescriptionAndIncludedProcesses": [{"value": "Der Beton wird aus Splitt und Sand (Zuschlagsstoffe), Wasser, hydraulischen Bindemitteln (Zement), Zusatzmitteln und Zusatzstoffen hergestellt. Die Kunststoffdübel werden in der Schalungsbahn fixiert und der Spannstahl vorgespannt. Anschließend wird der Beton von der Zentralmischanlage mittels Kübelbahn zur jeweiligen Schalungsbahn transportiert. Die Betoniermaschine befüllt die Schalungsbahn mit dem Beton. Bei Bedarf wird anschließend die Besohlung auf der Unterseite der Schwelle aufgebracht (eingerüttelt). Nach der entsprechenden Aushärtezeit des Betons, Vorgabe ist die Erreichung der Mindestdruckfestigkeit, werden die Weichenbetonschwellen entschalt und auf die geforderten, über den Schlaungsplan vorab definierten Längen geschnitten. Anschließend erfolgt die Zwischenlagerung auf dem Werksgelände. Die Herstellung der Weichenbetonschwellen findet in einem geschlossenen Gebäude bei Raumtemperatur statt. \nTechnische Daten: \nDie vorliegende EPD bezieht sich auf die deklarierten Spannbeton-Weichenschwellen der TSF-A. \nDeklarierte Einheit: \nDie vorliegende Umwelt-Produktdeklaration bezieht sich auf eine deklarierte Einheit von 1 lfm durchschnittliche WS 220 Spannbeton-Weichenschwelle mit einem Gewicht von 169 kg/lfm und einem Volumen von 0,065 m³.", "lang": "de"}, {"value": "The concrete is made of gravel and sand (aggregates), water, cement (hydraulic binder), admixtures and additives. Plastic dowels are fixed in the formwork liner and the prestressed steel is clamped. The concrete is then transported from the central mixing plant to the respective formwork line by means of a bucket conveyor. A concreting machine fills the formwork line with the concrete. If necessary, the under sleeper pads are then directly applied to the bottom of the sleepers. After the rewuired hardening time of the concrete, with the requirement that the minimum compressive strength has been reached, the concrete turnout sleepers are demoulded and cut to the required lengths defined in advance in the liner plan. Subsequently, the sleepers are placed in an intermediate storage area on the production site. The concrete turnout sleepers are manufactured in a closed building at room temperature. \nTechnical data: \nThis EPD refers to the declared prestressed concrete turnout sleepers of TSF-A. \nDeclared unit: \nThis environmental product declaration refers to a declared unit of 1 linear metre (lm) average WS 220 concrete turnout sleeper with a weight of 169 kg/lm and a volume of 0,065 m³.", "lang": "en"}], "technologicalApplicability": [{"value": "Die deklarierte Spannbeton-Weichenschwellen finden vorwiegend in folgenden Bereichen eine Anwendung:\n\nim Hochgeschwindigkeitsverkehr\nim Mischverkehr (Personen- und Güterverkehr)\nim städtischen Nahverkehr (U-Bahn, Straßenbahn, Light Rail-Verkehr).", "lang": "de"}, {"value": "The declared prestressed concrete turnout sleepers of voestalpine Railway Systems GmbH are mainly used in the following types of railway traffic:\n\n▪ High-Speed Traffic\n\n▪ Mixed Traffic (passenger and freight traffic)▪ Urban Traffic (Metro and Tram).", "lang": "en"}]}}, "modellingAndValidation": {"LCIMethodAndAllocation": {"typeOfDataSet": "EPD", "referenceToLCAMethodDetails": [{"shortDescription": [{"value": "Betonfertigteile.pdf", "lang": "de"}], "type": "source data set", "refObjectId": "dfc7c807-440c-40ee-943c-85433336cd62"}], "other": {"anies": [{"name": "subType", "value": "average dataset"}]}}, "dataSourcesTreatmentAndRepresentativeness": {"referenceToDataSource": [{"shortDescription": [{"value": "GaBi Database (all versions)", "lang": "de"}], "type": "source data set", "refObjectId": "28d74cc0-db8b-4d7e-bc44-5f6d56ce0c4a"}, {"shortDescription": [{"value": "GaBi database SP40 2020", "lang": "de"}], "type": "source data set", "refObjectId": "0115289e-52f0-4920-bc7e-57b1c96aec8d"}], "useAdviceForDataSet": [{"value": "Gültigkeitsbereich: \nDie vorliegende Umwelt-Produktdeklaration bezieht sich auf eine deklarierten Einheit von 1 lfm durchschnittliche Spannbeton-Weichenschwelle produziert am Standort der TSF-A GmbH in Sollenau (Österreich). \nSystemgrenze: \nDie Ökobilanz der Spannbeton-Weichenschwellen beinhaltet eine cradle-to-gate (Wiege bis zum Werkstor) ­Betrachtung mit Modulen. Die folgenden Lebenszyklusphasen werden in der Analyse berücksichtigt:\n\nModul A1-A3 | Produktionsstadium \n\nDas Produktionsstadium beinhaltet die Aufwendungen der Rohstoffversorgung (Beton, Splitt, Sand, Wasser, Spannstahl etc.) sowie der damit verbundenen Transporte bezogen auf den Produktionsstandort der TSF-A GmbH in Sollenau, Österreich. Die Produktionsstätte wird mit Strom aus dem regionalen Stromnetz und thermischer Energie aus Erdgas versorgt. Der Spannstahl wird von vorgelagerten Organisationen geliefert, die Teil des voestalpine-Konzerns sind. Somit werden die vorgelagerten Umweltwirkungen des gelieferten Stahls durch Primärdaten der jeweiligen Produktionsstandorte abgebildet. \n\n\nModul C1 | Rückbau/Abriss\n\nDer Energiebedarf für den Rückbau der Weichenschwellen aus dem Gleis (z. B. Lösen von Schrauben) ist stark von den Gegebenheiten vor Ort abhängig und wird als vernachlässigbar angesehen, wodurch keine Umweltwirkungen aus dem Rückbau der Produkte deklariert werden. \n\nModul C2 | Transport zur Abfallbehandlung \n\nModul C2 beinhaltet den Transport zur Abfallbehandlung. Dazu wird der Transport via LKW über 50 km Transportdistanz angesetzt. Dieses Szenario kann abhängig vom Ort des Rückbaus und der entsprechenden Abfallbehandlung variieren.\n\nModul C3 | Abfallbehandlung \n\nDas deklarierte Szenario geht von der Verarbeitung der Weichenschwellen in einem Betonbrecher aus. Es wird eine Verlustrate aus der Abfallverarbeitung von \n\n5 % angenommen. Entsprechende Umweltwirkungen werden in Modul C4 berücksichtigt. Die getrennten Materialfraktionen Stahl und Beton werden weiterverwertet. \n\nModul C4 | Beseitigung \n\nModul C4 beinhaltet die durch die Deponierung der Verluste aus der Abfallverarbeitung entstehenden Umweltwirkungen. Das gewählte Szenario beinhaltet daher die Umweltbelastungen der Deponierung von \n\n5 % des Materials. \n\nModul D | Gutschriften und Lasten außerhalb der Systemgrenzen \n\nModul D deklariert das Recycling des zurückgewonnenen Stahls und Betons (95 % des Produkts). Es beinhaltet das Potenzial zur Substitution von Primärstahl und Kies.", "lang": "de"}, {"value": "Scope: \nThis EPD is based on a declared unit of 1 linear metre (lm) of average concrete turnout sleeper, produced at the site TSF-A GmbH, Sollenau (Austria). \nSystem boundary: \nThe life cycle assessment of concrete turnout sleepers refers to a cradle-to-gate analysis with modules. Subsequent life cycle phases are part of the analysis:\n\nModule A1-A3 | Production stage\n\n\nThe production stage includes the upstream burdens of raw material supply (concrete, aggregates, sand, water, prestressing steel, etc.), their transports and the manufacturing at the production site of TSF-A GmbH located at Sollenau, Austria. The production site is supplied with electricity from the regional power grid and thermal energy from natural gas. The prestressing steel is delivered from upstream organisations which are part of voestalpine group. Thus, the upstream environmental impact of the steel supplied is represented by primary data of the respective production sites.  \n\n\n\nModule C1 | Deconstruction and demolition\n\nEnergy demand for the deconstruction of the sleepers from the track (e.g. loosening of screws) is strongly dependent on the conditions at site and considered to be negligible. This results in a declaration of “0” in module C1.\n\nModule C2 | Transport to disposal \n\nThe transport to the disposal of the material is estimated declaring a 50 km radius to the waste processing. This scenario may vary depending on the actual location of deconstruction and referring waste treatment. \n\nModule C3 | Waste processing \n\nThe declared scenario assumes the processing of the sleepers in a concrete breaker. Therefore, a loss rate from waste processing of 5 % is assumed. Referring environmental impacts are accounted for in module C4. The separated material fractions of steel and concrete are further recycled.  \n\nModule C4 | Disposal \n\nModule C4 refers to the emissions from the disposal of the losses from waste processing. The chosen scenario, therefore, includes the environmental burdens of landfilling of 5 % of the material.  \n\nModule D | Benefits and loads beyond the system boundary\n\n\nModule D declares the recycling of the recovered steel and concrete (95 % of the product). It includes the potential for substituting primary steel and gravel.", "lang": "en"}], "other": {"anies": [{"name": "referenceToOriginalEPD", "value": {"shortDescription": {"value": "Spannbeton-Weichenschwellen, TSF-A.pdf", "defaultValue": "Spannbeton-Weichenschwellen, TSF-A.pdf", "lstrings": [{"lang": "de", "value": "Spannbeton-Weichenschwellen, TSF-A.pdf"}]}, "type": "source data set", "uuid": {"uuid": "ab6079df-45ea-44c0-89fc-fd4d70139231"}, "refObjectId": "ab6079df-45ea-44c0-89fc-fd4d70139231", "resourceURLs": ["https://oekobaudat.de/OEKOBAU.DAT/resource/sources/ab6079df-45ea-44c0-89fc-fd4d70139231/Spannbeton-Weichenschwellen_TSF-A_14482.pdf?version=00.02.000"]}}]}}, "validation": {"review": [{"referenceToNameOfReviewerAndInstitution": [{"shortDescription": [{"value": "Institut Bauen und Umwelt e. V.", "lang": "de"}], "type": "contact data set", "refObjectId": "d111dbec-b024-4be5-86c5-752d6eb2cf95", "uri": "../contacts/d111dbec-b024-4be5-86c5-752d6eb2cf95.xml"}], "type": "Accredited third party review"}]}, "complianceDeclarations": {"compliance": [{"referenceToComplianceSystem": {"shortDescription": [{"value": "DIN EN 15804+A2", "lang": "de"}], "type": "source data set", "refObjectId": "c0016b33-8cf7-415c-ac6e-deba0d21440d", "uri": "../sources/c0016b33-8cf7-415c-ac6e-deba0d21440d.xml"}}, {"referenceToComplianceSystem": {"shortDescription": [{"value": "ISO 14025", "lang": "de"}], "type": "source data set", "refObjectId": "4f2eb655-6e44-4874-a95a-e28f5442cd4d", "uri": "../sources/4f2eb655-6e44-4874-a95a-e28f5442cd4d.xml"}}]}}, "administrativeInformation": {"commissionerAndGoal": {"referenceToCommissioner": [{"shortDescription": [{"value": "voestalpine AG", "lang": "de"}], "type": "contact data set", "refObjectId": "eef08a78-bb8b-429e-a968-c40f32a49ec7", "uri": "../contacts/eef08a78-bb8b-429e-a968-c40f32a49ec7.xml"}]}, "dataGenerator": {"referenceToPersonOrEntityGeneratingTheDataSet": [{"shortDescription": [{"value": "Daxner & Merl GmbH", "lang": "de"}], "type": "contact data set", "refObjectId": "ad8ad627-3991-42b7-a7ca-5a3fe0a34c28", "uri": "../contacts/ad8ad627-3991-42b7-a7ca-5a3fe0a34c28.xml"}]}, "dataEntryBy": {"timeStamp": 1625149323113, "referenceToDataSetFormat": [{"shortDescription": [{"value": "ILCD Format", "lang": "de"}], "type": "source data set", "refObjectId": "a97a0155-0234-4b87-b4ce-a45da52f2a40", "uri": "../sources/a97a0155-0234-4b87-b4ce-a45da52f2a40.xml"}, {"shortDescription": [{"value": "EPD-Datenformaterweiterungen v1.2", "lang": "de"}, {"value": "EPD Data Format Extensions v1.2", "lang": "en"}], "type": "source data set", "refObjectId": "a29449fd-aa2f-4de8-b5d7-4b06b43c6fde", "uri": "../sources/a29449fd-aa2f-4de8-b5d7-4b06b43c6fde.xml"}]}, "publicationAndOwnership": {"dataSetVersion": "00.02.000", "referenceToRegistrationAuthority": {"shortDescription": [{"value": "Institut Bauen und Umwelt e. V.", "lang": "de"}], "type": "contact data set", "refObjectId": "d111dbec-b024-4be5-86c5-752d6eb2cf95", "uri": "../contacts/d111dbec-b024-4be5-86c5-752d6eb2cf95.xml"}, "registrationNumber": "EPD-VRS-20210080-ICC1-DE", "referenceToOwnershipOfDataSet": {"shortDescription": [{"value": "voestalpine AG", "lang": "de"}], "type": "contact data set", "refObjectId": "eef08a78-bb8b-429e-a968-c40f32a49ec7", "uri": "../contacts/eef08a78-bb8b-429e-a968-c40f32a49ec7.xml"}, "copyright": true, "licenseType": "Free of charge for all users and uses", "accessRestrictions": [{"value": "None", "lang": "en"}], "other": {"anies": [{"name": "referenceToPublisher", "value": {"shortDescription": [{"value": "Institut Bauen und Umwelt e. V.", "lang": "de"}], "type": "contact data set", "refObjectId": "d111dbec-b024-4be5-86c5-752d6eb2cf95", "uri": "../contacts/d111dbec-b024-4be5-86c5-752d6eb2cf95.xml"}}]}}}, "exchanges": {"exchange": [{"dataSetInternalID": 0, "referenceToFlowDataSet": {"shortDescription": [{"value": "Spannbeton-Weichenschwelle (Spannbeton-Weichenschwelle)", "lang": "de"}], "type": "flow data set", "refObjectId": "c5fc76a2-b88e-85ec-058d-3d2432618d80", "uri": "../flows/c5fc76a2-b88e-85ec-058d-3d2432618d80.xml"}, "meanAmount": 1.0, "referencesToDataSource": {}, "referenceFlow": true, "resolvedFlowVersion": "00.02.000", "resultingflowAmount": 1.0, "flowProperties": [{"name": [{"lang": "en", "value": "Length"}, {"lang": "de", "value": "Länge"}], "uuid": "838aaa23-0117-11db-92e3-0800200c9a66", "referenceFlowProperty": true, "meanValue": 1.0, "referenceUnit": "m", "unitGroupUUID": "838aaa22-0117-11db-92e3-0800200c9a66"}], "materialProperties": [{"name": "gross density", "value": "2550.0", "unit": "kg/m^3", "unitDescription": "kilograms per cubic metre"}, {"name": "linear density", "value": "169.0", "unit": "kg/m"}, {"name": "mass reference", "value": "169.0", "unit": "kg/m^3", "unitDescription": "Kilogram per cubic meter "}, {"name": "conversion factor [mass/declared unit]", "value": "169.0", "unit": "-", "unitDescription": "Without unit"}], "typeOfFlow": "Product flow", "classification": {"classHierarchy": "Mineralische Baustoffe / Mörtel und Beton / Beton", "name": "OEKOBAU.DAT"}}, {"dataSetInternalID": 1, "referenceToFlowDataSet": {"shortDescription": [{"value": "Erneuerbare Primärenergie als Energieträger (PERE)", "lang": "de"}, {"value": "Renewable primary energy as energy carrier (PERE)", "lang": "en"}], "type": "flow data set", "refObjectId": "20f32be5-0398-4288-9b6d-accddd195317", "uri": "../flows/20f32be5-0398-4288-9b6d-accddd195317.xml"}, "exchange direction": "INPUT", "other": {"anies": [{"name": "referenceToUnitGroupDataSet", "value": {"shortDescription": [{"value": "MJ", "lang": "de"}], "type": "unit group data set", "refObjectId": "93a60a57-a3c8-11da-a746-0800200c9a66", "uri": "../unitgroups/93a60a57-a3c8-11da-a746-0800200c9a66.xml"}}, {"value": "43.4", "module": "A1-A3"}, {"value": "0", "module": "C1"}, {"value": "0.388", "module": "C2"}, {"value": "1.06", "module": "C3"}, {"value": "0.228", "module": "C4"}, {"value": "-5.77735606382883", "module": "D"}]}, "resolvedFlowVersion": "38.00.000", "flowProperties": [], "typeOfFlow": "Other flow", "classification": {"classHierarchy": "Quantities", "name": "GaBiCategories"}}, {"dataSetInternalID": 2, "referenceToFlowDataSet": {"shortDescription": [{"value": "Erneuerbare Primärenergie zur stofflichen Nutzung (PERM)", "lang": "de"}, {"value": "Renewable primary energy resources as material utilization (PERM)", "lang": "en"}], "type": "flow data set", "refObjectId": "fb3ec0de-548d-4508-aea5-00b73bf6f702", "uri": "../flows/fb3ec0de-548d-4508-aea5-00b73bf6f702.xml"}, "exchange direction": "INPUT", "other": {"anies": [{"name": "referenceToUnitGroupDataSet", "value": {"shortDescription": [{"value": "MJ", "lang": "de"}], "type": "unit group data set", "refObjectId": "93a60a57-a3c8-11da-a746-0800200c9a66", "uri": "../unitgroups/93a60a57-a3c8-11da-a746-0800200c9a66.xml"}}, {"value": "0", "module": "A1-A3"}, {"value": "0", "module": "C1"}, {"value": "0", "module": "C2"}, {"value": "0", "module": "C3"}, {"value": "0", "module": "C4"}, {"value": "0", "module": "D"}]}, "resolvedFlowVersion": "38.00.000", "flowProperties": [], "typeOfFlow": "Other flow", "classification": {"classHierarchy": "Quantities", "name": "GaBiCategories"}}, {"dataSetInternalID": 3, "referenceToFlowDataSet": {"shortDescription": [{"value": "Total erneuerbare Primärenergie (PERT)", "lang": "de"}, {"value": "Total use of renewable primary energy resources (PERT)", "lang": "en"}], "type": "flow data set", "refObjectId": "53f97275-fa8a-4cdd-9024-65936002acd0", "uri": "../flows/53f97275-fa8a-4cdd-9024-65936002acd0.xml"}, "exchange direction": "INPUT", "other": {"anies": [{"name": "referenceToUnitGroupDataSet", "value": {"shortDescription": [{"value": "MJ", "lang": "de"}], "type": "unit group data set", "refObjectId": "93a60a57-a3c8-11da-a746-0800200c9a66", "uri": "../unitgroups/93a60a57-a3c8-11da-a746-0800200c9a66.xml"}}, {"value": "43.4", "module": "A1-A3"}, {"value": "0", "module": "C1"}, {"value": "0.388", "module": "C2"}, {"value": "1.06", "module": "C3"}, {"value": "0.228", "module": "C4"}, {"value": "-5.77735606382883", "module": "D"}]}, "resolvedFlowVersion": "38.00.000", "flowProperties": [], "typeOfFlow": "Other flow", "classification": {"classHierarchy": "Quantities / Environmental quantities / EPD EN 15804 / LCI indicators", "name": "GaBiCategories"}}, {"dataSetInternalID": 4, "referenceToFlowDataSet": {"shortDescription": [{"value": "Nicht-erneuerbare Primärenergie als Energieträger (PENRE)", "lang": "de"}, {"value": "Non renewable primary energy as energy carrier (PENRE)", "lang": "en"}], "type": "flow data set", "refObjectId": "ac857178-2b45-46ec-892a-a9a4332f0372", "uri": "../flows/ac857178-2b45-46ec-892a-a9a4332f0372.xml"}, "exchange direction": "INPUT", "other": {"anies": [{"name": "referenceToUnitGroupDataSet", "value": {"shortDescription": [{"value": "MJ", "lang": "de"}], "type": "unit group data set", "refObjectId": "93a60a57-a3c8-11da-a746-0800200c9a66", "uri": "../unitgroups/93a60a57-a3c8-11da-a746-0800200c9a66.xml"}}, {"value": "318", "module": "A1-A3"}, {"value": "0", "module": "C1"}, {"value": "6.74", "module": "C2"}, {"value": "2.39", "module": "C3"}, {"value": "1.85", "module": "C4"}, {"value": "-72.8549113380311", "module": "D"}]}, "resolvedFlowVersion": "38.00.000", "flowProperties": [], "typeOfFlow": "Other flow", "classification": {"classHierarchy": "Quantities", "name": "GaBiCategories"}}, {"dataSetInternalID": 5, "referenceToFlowDataSet": {"shortDescription": [{"value": "Nicht-erneuerbare Primärenergie zur stofflichen Nutzung (PENRM)", "lang": "de"}, {"value": "Non renewable primary energy as material utilization (PENRM)", "lang": "en"}], "type": "flow data set", "refObjectId": "1421caa0-679d-4bf4-b282-0eb850ccae27", "uri": "../flows/1421caa0-679d-4bf4-b282-0eb850ccae27.xml"}, "exchange direction": "INPUT", "other": {"anies": [{"name": "referenceToUnitGroupDataSet", "value": {"shortDescription": [{"value": "MJ", "lang": "de"}], "type": "unit group data set", "refObjectId": "93a60a57-a3c8-11da-a746-0800200c9a66", "uri": "../unitgroups/93a60a57-a3c8-11da-a746-0800200c9a66.xml"}}, {"value": "3.4", "module": "A1-A3"}, {"value": "0", "module": "C1"}, {"value": "0", "module": "C2"}, {"value": "0", "module": "C3"}, {"value": "0", "module": "C4"}, {"value": "0", "module": "D"}]}, "resolvedFlowVersion": "38.00.000", "flowProperties": [], "typeOfFlow": "Other flow", "classification": {"classHierarchy": "Quantities", "name": "GaBiCategories"}}, {"dataSetInternalID": 6, "referenceToFlowDataSet": {"shortDescription": [{"value": "Total nicht erneuerbare Primärenergie (PENRT)", "lang": "de"}, {"value": "Total use of non renewable primary energy resources (PENRT)", "lang": "en"}], "type": "flow data set", "refObjectId": "06159210-646b-4c8d-8583-da9b3b95a6c1", "uri": "../flows/06159210-646b-4c8d-8583-da9b3b95a6c1.xml"}, "exchange direction": "INPUT", "other": {"anies": [{"name": "referenceToUnitGroupDataSet", "value": {"shortDescription": [{"value": "MJ", "lang": "de"}], "type": "unit group data set", "refObjectId": "93a60a57-a3c8-11da-a746-0800200c9a66", "uri": "../unitgroups/93a60a57-a3c8-11da-a746-0800200c9a66.xml"}}, {"value": "322", "module": "A1-A3"}, {"value": "0", "module": "C1"}, {"value": "6.74", "module": "C2"}, {"value": "2.39", "module": "C3"}, {"value": "1.85", "module": "C4"}, {"value": "-72.8549113380311", "module": "D"}]}, "resolvedFlowVersion": "38.00.000", "flowProperties": [], "typeOfFlow": "Other flow", "classification": {"classHierarchy": "Quantities / Environmental quantities / EPD EN 15804 / LCI indicators", "name": "GaBiCategories"}}, {"dataSetInternalID": 7, "referenceToFlowDataSet": {"shortDescription": [{"value": "Einsatz von Sekundärstoffen (SM)", "lang": "de"}, {"value": "Use of secondary material (SM)", "lang": "en"}], "type": "flow data set", "refObjectId": "c6a1f35f-2d09-4f54-8dfb-97e502e1ce92", "uri": "../flows/c6a1f35f-2d09-4f54-8dfb-97e502e1ce92.xml"}, "exchange direction": "INPUT", "other": {"anies": [{"name": "referenceToUnitGroupDataSet", "value": {"shortDescription": [{"value": "kg", "lang": "de"}], "type": "unit group data set", "refObjectId": "ad38d542-3fe9-439d-9b95-2f5f7752acaf", "uri": "../unitgroups/ad38d542-3fe9-439d-9b95-2f5f7752acaf.xml"}}, {"value": "3.36", "module": "A1-A3"}, {"value": "0", "module": "C1"}, {"value": "0", "module": "C2"}, {"value": "0", "module": "C3"}, {"value": "0", "module": "C4"}, {"value": "153.828083", "module": "D"}]}, "resolvedFlowVersion": "38.00.000", "flowProperties": [], "typeOfFlow": "Other flow", "classification": {"classHierarchy": "Quantities / Environmental quantities / EPD EN 15804 / LCI indicators", "name": "GaBiCategories"}}, {"dataSetInternalID": 8, "referenceToFlowDataSet": {"shortDescription": [{"value": "Erneuerbare Sekundärbrennstoffe (RSF)", "lang": "de"}, {"value": "Use of renewable secondary fuels (RSF)", "lang": "en"}], "type": "flow data set", "refObjectId": "64333088-a55f-4aa2-9a31-c10b07816787", "uri": "../flows/64333088-a55f-4aa2-9a31-c10b07816787.xml"}, "exchange direction": "INPUT", "other": {"anies": [{"name": "referenceToUnitGroupDataSet", "value": {"shortDescription": [{"value": "MJ", "lang": "de"}], "type": "unit group data set", "refObjectId": "93a60a57-a3c8-11da-a746-0800200c9a66", "uri": "../unitgroups/93a60a57-a3c8-11da-a746-0800200c9a66.xml"}}, {"value": "0", "module": "A1-A3"}, {"value": "0", "module": "C1"}, {"value": "0", "module": "C2"}, {"value": "0", "module": "C3"}, {"value": "0", "module": "C4"}, {"value": "0", "module": "D"}]}, "resolvedFlowVersion": "38.00.000", "flowProperties": [], "typeOfFlow": "Other flow", "classification": {"classHierarchy": "Quantities / Environmental quantities / EPD EN 15804 / LCI indicators", "name": "GaBiCategories"}}, {"dataSetInternalID": 9, "referenceToFlowDataSet": {"shortDescription": [{"value": "Nicht erneuerbare Sekundärbrennstoffe (NRSF)", "lang": "de"}, {"value": "Use of non renewable secondary fuels (NRSF)", "lang": "en"}], "type": "flow data set", "refObjectId": "89def144-d39a-4287-b86f-efde453ddcb2", "uri": "../flows/89def144-d39a-4287-b86f-efde453ddcb2.xml"}, "exchange direction": "INPUT", "other": {"anies": [{"name": "referenceToUnitGroupDataSet", "value": {"shortDescription": [{"value": "MJ", "lang": "de"}], "type": "unit group data set", "refObjectId": "93a60a57-a3c8-11da-a746-0800200c9a66", "uri": "../unitgroups/93a60a57-a3c8-11da-a746-0800200c9a66.xml"}}, {"value": "0", "module": "A1-A3"}, {"value": "0", "module": "C1"}, {"value": "0", "module": "C2"}, {"value": "0", "module": "C3"}, {"value": "0", "module": "C4"}, {"value": "0", "module": "D"}]}, "resolvedFlowVersion": "38.00.000", "flowProperties": [], "typeOfFlow": "Other flow", "classification": {"classHierarchy": "Quantities / Environmental quantities / EPD EN 15804 / LCI indicators", "name": "GaBiCategories"}}, {"dataSetInternalID": 10, "referenceToFlowDataSet": {"shortDescription": [{"value": "Einsatz von Süßwasserressourcen (FW)", "lang": "de"}, {"value": "Use of net fresh water (FW)", "lang": "en"}], "type": "flow data set", "refObjectId": "3cf952c8-f3a4-461d-8c96-96456ca62246", "uri": "../flows/3cf952c8-f3a4-461d-8c96-96456ca62246.xml"}, "exchange direction": "INPUT", "other": {"anies": [{"name": "referenceToUnitGroupDataSet", "value": {"shortDescription": [{"value": "m^3", "lang": "de"}], "type": "unit group data set", "refObjectId": "cd950537-0a98-4044-9ba7-9f9a68d0a504", "uri": "../unitgroups/cd950537-0a98-4044-9ba7-9f9a68d0a504.xml"}}, {"value": "0.0616", "module": "A1-A3"}, {"value": "0", "module": "C1"}, {"value": "0.000452", "module": "C2"}, {"value": "0.00123", "module": "C3"}, {"value": "0.00041", "module": "C4"}, {"value": "-0.0421413547342446", "module": "D"}]}, "resolvedFlowVersion": "38.00.000", "flowProperties": [], "typeOfFlow": "Other flow", "classification": {"classHierarchy": "Quantities / Environmental quantities / EPD EN 15804 / LCI indicators", "name": "GaBiCategories"}}, {"dataSetInternalID": 11, "referenceToFlowDataSet": {"shortDescription": [{"value": "Gefährlicher Abfall zur Deponie (HWD)", "lang": "de"}, {"value": "Hazardous waste disposed (HWD)", "lang": "en"}], "type": "flow data set", "refObjectId": "430f9e0f-59b2-46a0-8e0d-55e0e84948fc", "uri": "../flows/430f9e0f-59b2-46a0-8e0d-55e0e84948fc.xml"}, "exchange direction": "OUTPUT", "other": {"anies": [{"name": "referenceToUnitGroupDataSet", "value": {"shortDescription": [{"value": "kg", "lang": "de"}], "type": "unit group data set", "refObjectId": "ad38d542-3fe9-439d-9b95-2f5f7752acaf", "uri": "../unitgroups/ad38d542-3fe9-439d-9b95-2f5f7752acaf.xml"}}, {"value": "9.69E-07", "module": "A1-A3"}, {"value": "0", "module": "C1"}, {"value": "3.12E-07", "module": "C2"}, {"value": "9.9E-10", "module": "C3"}, {"value": "2.57E-08", "module": "C4"}, {"value": "-2.49E-07", "module": "D"}]}, "resolvedFlowVersion": "38.00.000", "flowProperties": [], "typeOfFlow": "Other flow", "classification": {"classHierarchy": "Quantities / Environmental quantities / EPD EN 15804 / LCI indicators", "name": "GaBiCategories"}}, {"dataSetInternalID": 12, "referenceToFlowDataSet": {"shortDescription": [{"value": "Entsorgter nicht gefährlicher Abfall (NHWD)", "lang": "de"}, {"value": "Non hazardous waste disposed (NHWD)", "lang": "en"}], "type": "flow data set", "refObjectId": "b29ef66b-e286-4afa-949f-62f1a7b4d7fa", "uri": "../flows/b29ef66b-e286-4afa-949f-62f1a7b4d7fa.xml"}, "exchange direction": "OUTPUT", "other": {"anies": [{"name": "referenceToUnitGroupDataSet", "value": {"shortDescription": [{"value": "kg", "lang": "de"}], "type": "unit group data set", "refObjectId": "ad38d542-3fe9-439d-9b95-2f5f7752acaf", "uri": "../unitgroups/ad38d542-3fe9-439d-9b95-2f5f7752acaf.xml"}}, {"value": "0.316", "module": "A1-A3"}, {"value": "0", "module": "C1"}, {"value": "0.00107", "module": "C2"}, {"value": "0.0017", "module": "C3"}, {"value": "8.46", "module": "C4"}, {"value": "0.526", "module": "D"}]}, "resolvedFlowVersion": "38.00.000", "flowProperties": [], "typeOfFlow": "Other flow", "classification": {"classHierarchy": "Quantities / Environmental quantities / EPD EN 15804 / LCI indicators", "name": "GaBiCategories"}}, {"dataSetInternalID": 13, "referenceToFlowDataSet": {"shortDescription": [{"value": "Entsorgter radioaktiver Abfall (RWD)", "lang": "de"}, {"value": "Radioactive waste disposed (RWD)", "lang": "en"}], "type": "flow data set", "refObjectId": "3449546e-52ad-4b39-b809-9fb77cea8ff6", "uri": "../flows/3449546e-52ad-4b39-b809-9fb77cea8ff6.xml"}, "exchange direction": "OUTPUT", "other": {"anies": [{"name": "referenceToUnitGroupDataSet", "value": {"shortDescription": [{"value": "kg", "lang": "de"}], "type": "unit group data set", "refObjectId": "ad38d542-3fe9-439d-9b95-2f5f7752acaf", "uri": "../unitgroups/ad38d542-3fe9-439d-9b95-2f5f7752acaf.xml"}}, {"value": "0.0111", "module": "A1-A3"}, {"value": "0", "module": "C1"}, {"value": "1.24E-05", "module": "C2"}, {"value": "0.000363", "module": "C3"}, {"value": "2.12E-05", "module": "C4"}, {"value": "-0.0033", "module": "D"}]}, "resolvedFlowVersion": "38.00.000", "flowProperties": [], "typeOfFlow": "Other flow", "classification": {"classHierarchy": "Quantities / Environmental quantities / EPD EN 15804 / LCI indicators", "name": "GaBiCategories"}}, {"dataSetInternalID": 14, "referenceToFlowDataSet": {"shortDescription": [{"value": "Komponenten für die Wiederverwendung (CRU)", "lang": "de"}, {"value": "Components for re-use (CRU)", "lang": "en"}], "type": "flow data set", "refObjectId": "a2b32f97-3fc7-4af2-b209-525bc6426f33", "uri": "../flows/a2b32f97-3fc7-4af2-b209-525bc6426f33.xml"}, "exchange direction": "OUTPUT", "other": {"anies": [{"name": "referenceToUnitGroupDataSet", "value": {"shortDescription": [{"value": "kg", "lang": "de"}], "type": "unit group data set", "refObjectId": "ad38d542-3fe9-439d-9b95-2f5f7752acaf", "uri": "../unitgroups/ad38d542-3fe9-439d-9b95-2f5f7752acaf.xml"}}, {"value": "0", "module": "A1-A3"}, {"value": "0", "module": "C1"}, {"value": "0", "module": "C2"}, {"value": "0", "module": "C3"}, {"value": "0", "module": "C4"}, {"value": "0", "module": "D"}]}, "resolvedFlowVersion": "38.00.000", "flowProperties": [], "typeOfFlow": "Other flow", "classification": {"classHierarchy": "Quantities / Environmental quantities / EPD EN 15804 / LCI indicators", "name": "GaBiCategories"}}, {"dataSetInternalID": 15, "referenceToFlowDataSet": {"shortDescription": [{"value": "Stoffe zum Recycling (MFR)", "lang": "de"}, {"value": "Materials for recycling (MFR)", "lang": "en"}], "type": "flow data set", "refObjectId": "d7fe48a5-4103-49c8-9aae-b0b5dfdbd6ae", "uri": "../flows/d7fe48a5-4103-49c8-9aae-b0b5dfdbd6ae.xml"}, "exchange direction": "OUTPUT", "other": {"anies": [{"name": "referenceToUnitGroupDataSet", "value": {"shortDescription": [{"value": "kg", "lang": "de"}], "type": "unit group data set", "refObjectId": "ad38d542-3fe9-439d-9b95-2f5f7752acaf", "uri": "../unitgroups/ad38d542-3fe9-439d-9b95-2f5f7752acaf.xml"}}, {"value": "0", "module": "A1-A3"}, {"value": "0", "module": "C1"}, {"value": "0", "module": "C2"}, {"value": "157", "module": "C3"}, {"value": "0", "module": "C4"}, {"value": "0", "module": "D"}]}, "resolvedFlowVersion": "38.00.000", "flowProperties": [], "typeOfFlow": "Other flow", "classification": {"classHierarchy": "Quantities / Environmental quantities / EPD EN 15804 / LCI indicators", "name": "GaBiCategories"}}, {"dataSetInternalID": 16, "referenceToFlowDataSet": {"shortDescription": [{"value": "Stoffe für die Energierückgewinnung (MER)", "lang": "de"}, {"value": "Materials for energy recovery (MER)", "lang": "en"}], "type": "flow data set", "refObjectId": "59a9181c-3aaf-46ee-8b13-2b3723b6e447", "uri": "../flows/59a9181c-3aaf-46ee-8b13-2b3723b6e447.xml"}, "exchange direction": "OUTPUT", "other": {"anies": [{"name": "referenceToUnitGroupDataSet", "value": {"shortDescription": [{"value": "kg", "lang": "de"}], "type": "unit group data set", "refObjectId": "ad38d542-3fe9-439d-9b95-2f5f7752acaf", "uri": "../unitgroups/ad38d542-3fe9-439d-9b95-2f5f7752acaf.xml"}}, {"value": "0", "module": "A1-A3"}, {"value": "0", "module": "C1"}, {"value": "0", "module": "C2"}, {"value": "0", "module": "C3"}, {"value": "0", "module": "C4"}, {"value": "0", "module": "D"}]}, "resolvedFlowVersion": "38.00.000", "flowProperties": [], "typeOfFlow": "Other flow", "classification": {"classHierarchy": "Quantities / Environmental quantities / EPD EN 15804 / LCI indicators", "name": "GaBiCategories"}}, {"dataSetInternalID": 17, "referenceToFlowDataSet": {"shortDescription": [{"value": "Exportierte elektrische Energie (EEE)", "lang": "de"}, {"value": "Exported electrical energy (EEE)", "lang": "en"}], "type": "flow data set", "refObjectId": "4da0c987-2b76-40d6-9e9e-82a017aaaf29", "uri": "../flows/4da0c987-2b76-40d6-9e9e-82a017aaaf29.xml"}, "exchange direction": "OUTPUT", "other": {"anies": [{"name": "referenceToUnitGroupDataSet", "value": {"shortDescription": [{"value": "MJ", "lang": "de"}], "type": "unit group data set", "refObjectId": "93a60a57-a3c8-11da-a746-0800200c9a66", "uri": "../unitgroups/93a60a57-a3c8-11da-a746-0800200c9a66.xml"}}, {"value": "0", "module": "A1-A3"}, {"value": "0", "module": "C1"}, {"value": "0", "module": "C2"}, {"value": "0", "module": "C3"}, {"value": "0", "module": "C4"}, {"value": "0", "module": "D"}]}, "resolvedFlowVersion": "38.00.000", "flowProperties": [], "typeOfFlow": "Other flow", "classification": {"classHierarchy": "Quantities / Environmental quantities / EPD EN 15804 / LCI indicators", "name": "GaBiCategories"}}, {"dataSetInternalID": 18, "referenceToFlowDataSet": {"shortDescription": [{"value": "Exportierte thermische Energie (EET)", "lang": "de"}, {"value": "Exported thermal energy (EET)", "lang": "en"}], "type": "flow data set", "refObjectId": "98daf38a-7a79-46d3-9a37-2b7bd0955810", "uri": "../flows/98daf38a-7a79-46d3-9a37-2b7bd0955810.xml"}, "exchange direction": "OUTPUT", "other": {"anies": [{"name": "referenceToUnitGroupDataSet", "value": {"shortDescription": [{"value": "MJ", "lang": "de"}], "type": "unit group data set", "refObjectId": "93a60a57-a3c8-11da-a746-0800200c9a66", "uri": "../unitgroups/93a60a57-a3c8-11da-a746-0800200c9a66.xml"}}, {"value": "0", "module": "A1-A3"}, {"value": "0", "module": "C1"}, {"value": "0", "module": "C2"}, {"value": "0", "module": "C3"}, {"value": "0", "module": "C4"}, {"value": "0", "module": "D"}]}, "resolvedFlowVersion": "38.00.000", "flowProperties": [], "typeOfFlow": "Other flow", "classification": {"classHierarchy": "Quantities / Environmental quantities / EPD EN 15804 / LCI indicators", "name": "GaBiCategories"}}]}, "LCIAResults": {"LCIAResult": [{"referenceToLCIAMethodDataSet": {"shortDescription": [{"value": "Globales Erwärmungspotenzial total (GWP-total)", "lang": "de"}, {"value": "Global Warming Potential total (GWP-total)", "lang": "en"}], "type": "LCIA method data set", "refObjectId": "6a37f984-a4b3-458a-a20a-64418c145fa2", "uri": "../lciamethods/6a37f984-a4b3-458a-a20a-64418c145fa2.xml"}, "other": {"anies": [{"name": "referenceToUnitGroupDataSet", "value": {"shortDescription": [{"value": "kg CO_(2)-Äq.", "lang": "de"}], "type": "unit group data set", "refObjectId": "1ebf3012-d0db-4de2-aefd-ef30cedb0be1", "uri": "../unitgroups/1ebf3012-d0db-4de2-aefd-ef30cedb0be1.xml"}}, {"value": "42", "module": "A1-A3"}, {"value": "0", "module": "C1"}, {"value": "0.509", "module": "C2"}, {"value": "0.137", "module": "C3"}, {"value": "0.13", "module": "C4"}, {"value": "-6.87", "module": "D"}]}}, {"referenceToLCIAMethodDataSet": {"shortDescription": [{"value": "Globales Erwärmungspotenzial fossil (GWP-fossil)", "lang": "de"}, {"value": "Global Warming Potential fossil fuels (GWP-fossil)", "lang": "en"}], "type": "LCIA method data set", "refObjectId": "5f635281-343e-44fb-83df-1971b155e6b6", "uri": "../lciamethods/5f635281-343e-44fb-83df-1971b155e6b6.xml"}, "other": {"anies": [{"name": "referenceToUnitGroupDataSet", "value": {"shortDescription": [{"value": "kg CO_(2)-Äq.", "lang": "de"}], "type": "unit group data set", "refObjectId": "1ebf3012-d0db-4de2-aefd-ef30cedb0be1", "uri": "../unitgroups/1ebf3012-d0db-4de2-aefd-ef30cedb0be1.xml"}}, {"value": "41.8", "module": "A1-A3"}, {"value": "0", "module": "C1"}, {"value": "0.506", "module": "C2"}, {"value": "0.136", "module": "C3"}, {"value": "0.14", "module": "C4"}, {"value": "-6.86", "module": "D"}]}}, {"referenceToLCIAMethodDataSet": {"shortDescription": [{"value": "Globales Erwärmungspotenzial biogen (GWP-biogenic)", "lang": "de"}, {"value": "Global Warming Potential biogenic (GWP-biogenic)", "lang": "en"}], "type": "LCIA method data set", "refObjectId": "2356e1ab-0185-4db5-86e5-16de51c7485c", "uri": "../lciamethods/2356e1ab-0185-4db5-86e5-16de51c7485c.xml"}, "other": {"anies": [{"name": "referenceToUnitGroupDataSet", "value": {"shortDescription": [{"value": "kg CO_(2)-Äq.", "lang": "de"}], "type": "unit group data set", "refObjectId": "1ebf3012-d0db-4de2-aefd-ef30cedb0be1", "uri": "../unitgroups/1ebf3012-d0db-4de2-aefd-ef30cedb0be1.xml"}}, {"value": "0.122", "module": "A1-A3"}, {"value": "0", "module": "C1"}, {"value": "-0.000845", "module": "C2"}, {"value": "0.000454", "module": "C3"}, {"value": "-0.0102", "module": "C4"}, {"value": "-0.00649", "module": "D"}]}}, {"referenceToLCIAMethodDataSet": {"shortDescription": [{"value": "Globales Erwärmungspotenzial luluc (GWP-luluc)", "lang": "de"}, {"value": "Global Warming Potential luluc (GWP-luluc)", "lang": "en"}], "type": "LCIA method data set", "refObjectId": "4331bbdb-978a-490d-8707-eeb047f01a55", "uri": "../lciamethods/4331bbdb-978a-490d-8707-eeb047f01a55.xml"}, "other": {"anies": [{"name": "referenceToUnitGroupDataSet", "value": {"shortDescription": [{"value": "kg CO_(2)-Äq.", "lang": "de"}], "type": "unit group data set", "refObjectId": "1ebf3012-d0db-4de2-aefd-ef30cedb0be1", "uri": "../unitgroups/1ebf3012-d0db-4de2-aefd-ef30cedb0be1.xml"}}, {"value": "0.0199", "module": "A1-A3"}, {"value": "0", "module": "C1"}, {"value": "0.00407", "module": "C2"}, {"value": "0.000197", "module": "C3"}, {"value": "0.00037", "module": "C4"}, {"value": "-0.00434", "module": "D"}]}}, {"referenceToLCIAMethodDataSet": {"shortDescription": [{"value": "Abbau Potential der stratosphärischen Ozonschicht (ODP)", "lang": "de"}, {"value": "Depletion potential of the stratospheric ozone layer (ODP)", "lang": "en"}], "type": "LCIA method data set", "refObjectId": "b5c629d6-def3-11e6-bf01-fe55135034f3", "uri": "../lciamethods/b5c629d6-def3-11e6-bf01-fe55135034f3.xml"}, "other": {"anies": [{"name": "referenceToUnitGroupDataSet", "value": {"shortDescription": [{"value": "kg CFC11-Äq.", "lang": "de"}], "type": "unit group data set", "refObjectId": "d9e957c9-7309-4474-bf3a-7777df6c4e5b", "uri": "../unitgroups/d9e957c9-7309-4474-bf3a-7777df6c4e5b.xml"}}, {"value": "4.38E-09", "module": "A1-A3"}, {"value": "0", "module": "C1"}, {"value": "9.23E-17", "module": "C2"}, {"value": "2.99E-15", "module": "C3"}, {"value": "4.93E-16", "module": "C4"}, {"value": "-3.59E-14", "module": "D"}]}}, {"referenceToLCIAMethodDataSet": {"shortDescription": [{"value": "Versauerungspotenzial von Boden und Wasser (AP)", "lang": "de"}, {"value": "Acidification potential of land and water (AP)", "lang": "en"}], "type": "LCIA method data set", "refObjectId": "b5c611c6-def3-11e6-bf01-fe55135034f3", "uri": "../lciamethods/b5c611c6-def3-11e6-bf01-fe55135034f3.xml"}, "other": {"anies": [{"name": "referenceToUnitGroupDataSet", "value": {"shortDescription": [{"value": "mol H^(+)-Äq.", "lang": "de"}], "type": "unit group data set", "refObjectId": "42e089ac-92bf-4bf2-8ca1-5fc40d18f2ed", "uri": "../unitgroups/42e089ac-92bf-4bf2-8ca1-5fc40d18f2ed.xml"}}, {"value": "0.0948", "module": "A1-A3"}, {"value": "0", "module": "C1"}, {"value": "0.00171", "module": "C2"}, {"value": "0.0003", "module": "C3"}, {"value": "0.000936", "module": "C4"}, {"value": "-0.0135", "module": "D"}]}}, {"referenceToLCIAMethodDataSet": {"shortDescription": [{"value": "Eutrophierungspotenzial Süßwasser (EP-freshwater)", "lang": "de"}, {"value": "Eutrophication potential aquatic freshwater (EP-freshwater)", "lang": "en"}], "type": "LCIA method data set", "refObjectId": "b53ec18f-7377-4ad3-86eb-cc3f4f276b2b", "uri": "../lciamethods/b53ec18f-7377-4ad3-86eb-cc3f4f276b2b.xml"}, "other": {"anies": [{"name": "referenceToUnitGroupDataSet", "value": {"shortDescription": [{"value": "kg PO_(4)-Äq.", "lang": "de"}], "type": "unit group data set", "refObjectId": "0429039d-a61d-4590-ba67-aa4a20a810a1", "uri": "../unitgroups/0429039d-a61d-4590-ba67-aa4a20a810a1.xml"}}, {"value": "0.000123", "module": "A1-A3"}, {"value": "0", "module": "C1"}, {"value": "1.53E-06", "module": "C2"}, {"value": "3.63E-07", "module": "C3"}, {"value": "2.24E-07", "module": "C4"}, {"value": "-5.62E-06", "module": "D"}]}}, {"referenceToLCIAMethodDataSet": {"shortDescription": [{"value": "Eutrophierungspotenzial Salzwasser (EP-marine)", "lang": "de"}, {"value": "Eutrophication potential aquatic marine (EP-marine)", "lang": "en"}], "type": "LCIA method data set", "refObjectId": "b5c619fa-def3-11e6-bf01-fe55135034f3", "uri": "../lciamethods/b5c619fa-def3-11e6-bf01-fe55135034f3.xml"}, "other": {"anies": [{"name": "referenceToUnitGroupDataSet", "value": {"shortDescription": [{"value": "kg N-Äq.", "lang": "de"}], "type": "unit group data set", "refObjectId": "d05bb823-ecdf-4686-8c40-bf1d9257859f", "uri": "../unitgroups/d05bb823-ecdf-4686-8c40-bf1d9257859f.xml"}}, {"value": "0.0279", "module": "A1-A3"}, {"value": "0", "module": "C1"}, {"value": "0.000771", "module": "C2"}, {"value": "6.67E-05", "module": "C3"}, {"value": "0.00024", "module": "C4"}, {"value": "-0.00261", "module": "D"}]}}, {"referenceToLCIAMethodDataSet": {"shortDescription": [{"value": "Eutrophierungspotenzial Land (EP-terrestrial)", "lang": "de"}, {"value": "Eutrophication potential terrestrial (EP-terrestrial)", "lang": "en"}], "type": "LCIA method data set", "refObjectId": "b5c614d2-def3-11e6-bf01-fe55135034f3", "uri": "../lciamethods/b5c614d2-def3-11e6-bf01-fe55135034f3.xml"}, "other": {"anies": [{"name": "referenceToUnitGroupDataSet", "value": {"shortDescription": [{"value": "mol N-Äq.", "lang": "de"}], "type": "unit group data set", "refObjectId": "71b4d617-0ec9-4d3f-b65e-e438940c2401", "uri": "../unitgroups/71b4d617-0ec9-4d3f-b65e-e438940c2401.xml"}}, {"value": "0.302", "module": "A1-A3"}, {"value": "0", "module": "C1"}, {"value": "0.00862", "module": "C2"}, {"value": "0.000701", "module": "C3"}, {"value": "0.00264", "module": "C4"}, {"value": "-0.0273", "module": "D"}]}}, {"referenceToLCIAMethodDataSet": {"shortDescription": [{"value": "Bildungspotential für troposphärisches Ozon (POCP)", "lang": "de"}, {"value": "Formation potential of tropospheric ozone photochemical oxidants (POCP)", "lang": "en"}], "type": "LCIA method data set", "refObjectId": "b5c610fe-def3-11e6-bf01-fe55135034f3", "uri": "../lciamethods/b5c610fe-def3-11e6-bf01-fe55135034f3.xml"}, "other": {"anies": [{"name": "referenceToUnitGroupDataSet", "value": {"shortDescription": [{"value": "kg NMVOC-Äq.", "lang": "de"}], "type": "unit group data set", "refObjectId": "d27c25f8-fbc1-44c6-b47b-4adbae4199c6", "uri": "../unitgroups/d27c25f8-fbc1-44c6-b47b-4adbae4199c6.xml"}}, {"value": "0.0857", "module": "A1-A3"}, {"value": "0", "module": "C1"}, {"value": "0.00152", "module": "C2"}, {"value": "0.000183", "module": "C3"}, {"value": "0.000729", "module": "C4"}, {"value": "-0.0103", "module": "D"}]}}, {"referenceToLCIAMethodDataSet": {"shortDescription": [{"value": "Potenzial für den abiotischen Abbau nicht fossiler Ressourcen (ADPE)", "lang": "de"}, {"value": "Abiotic depletion potential for non fossil resources (ADPE)", "lang": "en"}], "type": "LCIA method data set", "refObjectId": "b2ad6494-c78d-11e6-9d9d-cec0c932ce01", "uri": "../lciamethods/b2ad6494-c78d-11e6-9d9d-cec0c932ce01.xml"}, "other": {"anies": [{"name": "referenceToUnitGroupDataSet", "value": {"shortDescription": [{"value": "kg Sb-Äq.", "lang": "de"}], "type": "unit group data set", "refObjectId": "54ccd2d9-a32a-4fc2-923d-f2c8c93e89d4", "uri": "../unitgroups/54ccd2d9-a32a-4fc2-923d-f2c8c93e89d4.xml"}}, {"value": "2.18E-05", "module": "A1-A3"}, {"value": "0", "module": "C1"}, {"value": "4.07E-08", "module": "C2"}, {"value": "3.94E-08", "module": "C3"}, {"value": "1.22E-08", "module": "C4"}, {"value": "-1.17E-05", "module": "D"}]}}, {"referenceToLCIAMethodDataSet": {"shortDescription": [{"value": "Potenzial für den abiotischen Abbau fossiler Brennstoffe (ADPF)", "lang": "de"}, {"value": "Abiotic depletion potential for fossil resources (ADPF)", "lang": "en"}], "type": "LCIA method data set", "refObjectId": "b2ad6110-c78d-11e6-9d9d-cec0c932ce01", "uri": "../lciamethods/b2ad6110-c78d-11e6-9d9d-cec0c932ce01.xml"}, "other": {"anies": [{"name": "referenceToUnitGroupDataSet", "value": {"shortDescription": [{"value": "MJ", "lang": "de"}], "type": "unit group data set", "refObjectId": "93a60a57-a3c8-11da-a746-0800200c9a66", "uri": "../unitgroups/93a60a57-a3c8-11da-a746-0800200c9a66.xml"}}, {"value": "321", "module": "A1-A3"}, {"value": "0", "module": "C1"}, {"value": "6.71", "module": "C2"}, {"value": "2.39", "module": "C3"}, {"value": "1.85", "module": "C4"}, {"value": "-72.8", "module": "D"}]}}, {"referenceToLCIAMethodDataSet": {"shortDescription": [{"value": "Wassernutzung (WDP)", "lang": "de"}, {"value": "Water use (WDP)", "lang": "en"}], "type": "LCIA method data set", "refObjectId": "b2ad66ce-c78d-11e6-9d9d-cec0c932ce01", "uri": "../lciamethods/b2ad66ce-c78d-11e6-9d9d-cec0c932ce01.xml"}, "other": {"anies": [{"name": "referenceToUnitGroupDataSet", "value": {"shortDescription": [{"value": "m^(3) Welt-Äq. entzogen", "lang": "de"}], "type": "unit group data set", "refObjectId": "6ae2df01-888e-46c8-b17d-49fa3869b476", "uri": "../unitgroups/6ae2df01-888e-46c8-b17d-49fa3869b476.xml"}}, {"value": "2.06", "module": "A1-A3"}, {"value": "0", "module": "C1"}, {"value": "0.00491", "module": "C2"}, {"value": "0.0297", "module": "C3"}, {"value": "0.0127", "module": "C4"}, {"value": "-1.63", "module": "D"}]}}, {"referenceToLCIAMethodDataSet": {"shortDescription": [{"value": "Auftreten von Krankheiten aufgrund von Feinstaubemissionen (PM)", "lang": "de"}, {"value": "Incidence of disease due to PM emissions (PM)", "lang": "en"}], "type": "LCIA method data set", "refObjectId": "b5c602c6-def3-11e6-bf01-fe55135034f3", "uri": "../lciamethods/b5c602c6-def3-11e6-bf01-fe55135034f3.xml"}, "other": {"anies": [{"name": "referenceToUnitGroupDataSet", "value": {"shortDescription": [{"value": "Krankheitsfälle", "lang": "de"}], "type": "unit group data set", "refObjectId": "3883559b-648f-4afc-8ba2-0bd24f3affa3", "uri": "../unitgroups/3883559b-648f-4afc-8ba2-0bd24f3affa3.xml"}}, {"value": "3.86E-07", "module": "A1-A3"}, {"value": "0", "module": "C1"}, {"value": "4.35E-09", "module": "C2"}, {"value": "6.49E-10", "module": "C3"}, {"value": "1.52E-08", "module": "C4"}, {"value": "-1.48E-09", "module": "D"}]}}, {"referenceToLCIAMethodDataSet": {"shortDescription": [{"value": "Wirkung durch Exposition des Menschen mit U235 (IR)", "lang": "de"}, {"value": "Human exposure efficiency relative to U235 (IR)", "lang": "en"}], "type": "LCIA method data set", "refObjectId": "b5c632be-def3-11e6-bf01-fe55135034f3", "uri": "../lciamethods/b5c632be-def3-11e6-bf01-fe55135034f3.xml"}, "other": {"anies": [{"name": "referenceToUnitGroupDataSet", "value": {"shortDescription": [{"value": "kBq U235-Äq.", "lang": "de"}], "type": "unit group data set", "refObjectId": "456b05bf-1415-44a9-9993-02452f554c09", "uri": "../unitgroups/456b05bf-1415-44a9-9993-02452f554c09.xml"}}, {"value": "2.18E-09", "module": "A1-A3"}, {"value": "0", "module": "C1"}, {"value": "3.51E-11", "module": "C2"}, {"value": "1.14E-11", "module": "C3"}, {"value": "1.57E-11", "module": "C4"}, {"value": "-7.43E-10", "module": "D"}]}}, {"referenceToLCIAMethodDataSet": {"shortDescription": [{"value": "Toxizitätsvergleichseinheit für Ökosysteme (ETP-fw)", "lang": "de"}, {"value": "Comparative toxic unit for ecosystems (ETP-fw)", "lang": "en"}], "type": "LCIA method data set", "refObjectId": "ee1082d1-b0f7-43ca-a1f0-21e2a4a74511", "uri": "../lciamethods/ee1082d1-b0f7-43ca-a1f0-21e2a4a74511.xml"}, "other": {"anies": [{"name": "referenceToUnitGroupDataSet", "value": {"shortDescription": [{"value": "CTUe", "lang": "de"}], "type": "unit group data set", "refObjectId": "aa959ded-f1eb-4efb-9c5c-2d60be36b3e6", "uri": "../unitgroups/aa959ded-f1eb-4efb-9c5c-2d60be36b3e6.xml"}}, {"value": "1.24E-06", "module": "A1-A3"}, {"value": "0", "module": "C1"}, {"value": "9.66E-09", "module": "C2"}, {"value": "2.52E-09", "module": "C3"}, {"value": "1.15E-08", "module": "C4"}, {"value": "-2.64E-07", "module": "D"}]}}, {"referenceToLCIAMethodDataSet": {"shortDescription": [{"value": "Toxizitätsvergleichseinheit für Menschen (krebserregend) (HTP-c)", "lang": "de"}, {"value": "Comparative toxic unit for humans (carcinogenic) (HTP-c)", "lang": "en"}], "type": "LCIA method data set", "refObjectId": "2299222a-bbd8-474f-9d4f-4dd1f18aea7c", "uri": "../lciamethods/2299222a-bbd8-474f-9d4f-4dd1f18aea7c.xml"}, "other": {"anies": [{"name": "referenceToUnitGroupDataSet", "value": {"shortDescription": [{"value": "CTUh", "lang": "de"}], "type": "unit group data set", "refObjectId": "d4c9523e-2d7e-49fd-8469-998f547d3a70", "uri": "../unitgroups/d4c9523e-2d7e-49fd-8469-998f547d3a70.xml"}}, {"value": "1.71", "module": "A1-A3"}, {"value": "0", "module": "C1"}, {"value": "0.00183", "module": "C2"}, {"value": "0.0596", "module": "C3"}, {"value": "0.00229", "module": "C4"}, {"value": "-0.405", "module": "D"}]}}, {"referenceToLCIAMethodDataSet": {"shortDescription": [{"value": "Toxizitätsvergleichseinheit für Menschen (nicht krebserregend) (HTP-nc)", "lang": "de"}, {"value": "Comparative toxic unit for humans (noncarcinogenic) (HTP-nc)", "lang": "en"}], "type": "LCIA method data set", "refObjectId": "3af763a5-b7a1-48c9-9cee-1f223481fcef", "uri": "../lciamethods/3af763a5-b7a1-48c9-9cee-1f223481fcef.xml"}, "other": {"anies": [{"name": "referenceToUnitGroupDataSet", "value": {"shortDescription": [{"value": "CTUh", "lang": "de"}], "type": "unit group data set", "refObjectId": "d4c9523e-2d7e-49fd-8469-998f547d3a70", "uri": "../unitgroups/d4c9523e-2d7e-49fd-8469-998f547d3a70.xml"}}, {"value": "150", "module": "A1-A3"}, {"value": "0", "module": "C1"}, {"value": "5.02", "module": "C2"}, {"value": "1.02", "module": "C3"}, {"value": "0.993", "module": "C4"}, {"value": "-13.2", "module": "D"}]}}, {"referenceToLCIAMethodDataSet": {"shortDescription": [{"value": "Bodenqualitätsindex (SQP)", "lang": "de"}, {"value": "Soil quality index (SQP)", "lang": "en"}], "type": "LCIA method data set", "refObjectId": "b2ad6890-c78d-11e6-9d9d-cec0c932ce01", "uri": "../lciamethods/b2ad6890-c78d-11e6-9d9d-cec0c932ce01.xml"}, "other": {"anies": [{"name": "referenceToUnitGroupDataSet", "value": {"shortDescription": [{"value": "SQP", "lang": "de"}], "type": "unit group data set", "refObjectId": "f130951c-e67f-4f7f-8dd4-665de3974e18", "uri": "../unitgroups/f130951c-e67f-4f7f-8dd4-665de3974e18.xml"}}, {"value": "5.72E-09", "module": "A1-A3"}, {"value": "0", "module": "C1"}, {"value": "1.04E-10", "module": "C2"}, {"value": "2.83E-11", "module": "C3"}, {"value": "1.45E-10", "module": "C4"}, {"value": "1.38E-09", "module": "D"}]}}]}, "otherAttributes": {"{http://www.indata.network/EPD/2019}epd-version": "1.2"}, "version": "1.1", "locations": "../ILCDLocations.xml"}