{"processInformation": {"dataSetInformation": {"UUID": "80e3d34e-6f37-4d1d-94fd-b9694b96223d", "name": {"baseName": [{"value": "Electricity grid mix 2019", "lang": "en"}, {"value": "Strom für Gebäudebetrieb 2019", "lang": "de"}], "functionalUnitFlowProperties": [{"value": "<1kV", "lang": "en"}]}, "classificationInformation": {"classification": [{"class": [{"value": "Sonstige", "level": 0, "classId": "9"}, {"value": "Energieträger - Bereitstellung frei Verbraucher", "level": 1, "classId": "9.2"}, {"value": "Strom", "level": 2, "classId": "9.2.05"}], "name": "oekobau.dat"}]}, "generalComment": [{"value": "This data set has been modeled according to the European Standard EN 15804+A2 for Sustainable Building. Results are depicted in modules that allow the structured expression of results over the entire life cycle.", "lang": "en"}, {"value": "Dieser Datensatz wurde nach dem European Standard EN 15804+A2 für Nachhaltiges Bauen modelliert. Ergebnisse werden in Modulen abgebildet, die den strukturierten Ausdruck von Ergebnissen über den gesamten Lebenszyklus zulassen.", "lang": "de"}], "other": {"anies": [{"margins": 0, "description": [{"lang": "en"}, {"lang": "de"}]}]}}, "quantitativeReference": {"referenceToReferenceFlow": [100152], "type": "Reference flow(s)"}, "time": {"referenceYear": 2023, "dataSetValidUntil": 2026, "timeRepresentativenessDescription": [{"value": "Annual average", "lang": "en"}, {"value": "Jährlicher Durchschnitt", "lang": "de"}]}, "geography": {"locationOfOperationSupplyOrProduction": {"descriptionOfRestrictions": [{"value": "The data set represents the country specific situation in Germany, focusing on the main technologies, the region specific characteristics and / or import statistics.", "lang": "en"}, {"value": "Der Datensatz bildet die länderspezifische Situation in Deutschland ab. Dabei werden Haupttechnologien, spezifische regionale Charakteristiken und ggf. Importstatistiken berücksichtigt.", "lang": "de"}], "location": "DE"}}, "technology": {"technologyDescriptionAndIncludedProcesses": [{"value": "Foreground system:\nThe national or regional specific electricity consumption mix is provided by the conversion of the different energy carriers to electricity and imports from neighbouring countries, as illustrated in the pie chart \"Electricity Mix\".\nThe electricity is either produced in energy carrier specific power plants and/or combined heat and power plants (CHP). Also considered are the national and regional specific technology standards of the power plants in regard to efficiency, firing technology, flue-gas desulphurisation, NOx removal and de-dusting. The electricity provided by non-combustible renewable energy sources also considers the national or regional situation, such as solar radiation (photovoltaic), annual full load hours (wind power), and share of hydro power stations by type (run-of-river, storage and pumped storage).\nThe fossil power plant models combine emission data from literature with calculated values for non-measured emissions e.g. organics or heavy metals. For the emissions CO2, SO2, NOx, CO, CH4, N2O, NMVOC and particulate matter (PM) measured/calculated data are used, taken from national inventory reports, emission inventory data bases, utility companies and other sources. The calculation of other emissions within the models are based on energy carrier properties, transfer coefficients and power plant thermodynamics representing the applied flue gas treatment technologies and standards (flue gas desulphurisation, dust filter etc.). Combustion residues from solid fuels, such as gypsum, bottom ash or fly ash are assumed  to be reused e.g. in construction work. Waste treatment for these substances is therefore not considered. Radioactive emissions from ashes are not considered in the coal power plant model.\nThe energy carrier supply considers the whole supply chain of the energy carrier from exploration, production, processing and transport of the fuels to the power plants. The supply chain is modelled in specific national / regional energy carrier consumption mixes (i.e. domestic production and imports), and considers national / regional average energy carrier properties (e.g. elemental composition and energy content).\nThe electricity grid mix includes imported electricity from neighbouring countries, transmission / distribution losses of low voltage electricity supply and the own use of electricity by energy producers (own consumption of power plants, and \"other\" own consumption e.g. due to pumped storage hydro power etc.). The logic of modelling the electricity consumption mix is represented in the flow diagram \"Modelling of Electricity Consumption Mixes\".\nBackground system:\nElectricity: Electricity is modelled according to the individual country-specific situations. The country-specific modelling is achieved on multiple levels. Firstly, individual energy carrier specific power plants and plants for renewable energy sources are modelled according to the current national electricity grid mix. Modelling the electricity consumption mix includes transmission / distribution losses and the own use by energy producers (own consumption of power plants and \"other\" own consumption e.g. due to pumped storage hydro power etc.), as well as imported electricity. Secondly, the national emission and efficiency standards of the power plants are modelled as well as the share of electricity plants and combined heat and power plants (CHP). Thirdly, the country-specific energy carrier supply (share of imports and / or domestic supply) including the country-specific energy carrier properties (e.g. element and energy content) are accounted for. Fourthly, the exploration, mining/production, processing and transport processes of the energy carrier supply chains are modelled according to the specific situation of each electricity producing country. The different production and processing techniques (emissions and efficiencies) in the different energy producing countries are considered, e.g. different crude oil production technologies or different flaring rates at the oil platforms.\nThermal energy, process steam: The thermal energy and process steam supply is modelled according to the individual country-specific situation with regard to emission standards and considered energy carriers. The thermal energy and process steam are produced at heat plants. Efficiencies for thermal energy production are by definition 100% in relation to the corresponding energy carrier input. For process steam the efficiency ranges from 85%, 90% to 95%. The energy carriers used for the generation of thermal energy and process steam are modelled according to the specific import situation (see electricity above).\nTransports: All relevant and known transport processes are included. Ocean-going and inland ship transport as well as rail, truck and pipeline transport of bulk commodities are considered.\nEnergy carriers: The energy carriers are modelled according to the specific supply situation (see electricity above).\nRefinery products: Diesel fuel, gasoline, technical gases, fuel oils, lubricants and residues such as bitumen are modelled with a parameterised country-specific refinery model. The refinery model represents the current national standard in refining techniques (e.g. emission level, internal energy consumption, etc.) as well as the individual country-specific product output spectrum, which can be quite different from country to country. The supply of crude oil is modelled, again, according to the country-specific situation with the respective properties of the resources.", "lang": "en"}, {"value": "Vordergrundsystem:\nDer länder- bzw. regionsspezifische Strommix, der sich aus dem Einsatz der verschiedenen Energieträger zur Stromgewinnung ergibt, ist im Kreisdiagramm \"Strommix\" dargestellt. \nDer Strom wird in Elektrizitätskraftwerken und/oder in speziellen Kraftwerken mit Kraft-Wärme-Kopplung (KWK) erzeugt. Der Datensatz berücksichtigt länder- bzw. regionsspezifische Technologiestandards der Kraftwerke in Bezug auf Effizienz, Feuerungstechnik, Rauchgasentschwefelung, Entstickung und Entstaubung. Der durch erneuerbare Energien erzeugte Strom spiegelt ebenfalls die länder- bzw. regionsspezifische Situation wider, wie Sonneneinstrahlung (Photovoltaik), jährliche Volllaststunden (Windkraft) und Art der Wasserkraftwerke (Laufwasserkraftwerke, Speicher- und Pumpspeicherwerke).\nDie Kraftwerksmodelle auf Basis fossiler Energieträger nutzen sowohl Emissionsdaten aus der Literatur als auch berechnete Werte für nicht-messbare Emissionen, wie z. B. organischer Emissionen oder Schwermetallemissionen. Für die Emissionen von CO2, SO2, NOx, CO, CH4, N2O, NMVOC und Staub werden gemessene/berechnete Daten aus nationalen Statistiken, Emissionsdatenbanken, von Versorgungsunternehmen und aus anderen Quellen verwendet. Die Berechnung der übrigen Emissionen basiert auf den Eigenschaften der Energieträger, Transferkoeffizienten und thermodynamischen Grundsätzen. Die Anwendung von Standards der Rauchgasreinigung, wie Rauchgasentschwefelung, Staubfilterung etc. wird berücksichtigt. Es wird angenommen, dass Verbrennungsrückstände von festen Brennstoffen, wie z.B. Gips, Kessel- oder Flugasche, weiterverwendet werde, z. B. im Straßenbau. Die Abfallbehandlung für diese Stoffe wird daher nicht berücksichtigt. Radioaktive Emissionen aus der Asche sind im Kohlekraftwerk-Modell nicht berücksichtigt.\nDie Energieträgerbereitstellung berücksichtigt die gesamte Vorkette des Energieträgers von der Erschließung über die Produktion, Aufbereitung bis hin zum Transport der Energieträger zum Kraftwerk. Die Vorkette wird entsprechend der länder- bzw. regionsspezifischen Energieträgermixe modelliert (d. h. Eigenproduktion sowie Importe sind berücksichtigt) und bezieht die länder- bzw. regionsspezifischen durchschnittlichen Eigenschaften der Energieträger ein (z. B. Elementarzusammensetzung und Heizwert).\nDer Strommix beeinhaltet Stromimporte aus den Nachbarländern, Transmissions- und Verteilungsversluste, Eigenverbräuche der Stromerzeuger (Eigenverbräuche der Kraftwerke und \"andere\" Eigenverbräuche wie z.B. Pumpspeicherkraftwerke). Die Grundsätze der Modellierung des Strommixes sind in dem Flussdiagramm \"Modellierung des Strommixes\" dargestellt.\nHintergrundsystem:\nStrom: Die Stromerzeugung wird entsprechend der länderspezifischen Randbedingungen modelliert. Die landesspezifische Analyse beinhaltet:\n1. Spezifische Kraftwerke der verschiedenen fossilen Energieträger und der Einsatz erneuerbarer Energien sind entsprechend der länderspezifischen Energieträgermixe modelliert. Die Analyse bezieht Stromimporte aus den Nachbarländern, Transmissions-und Verteilungsverluste und den Eigenverbrauch im Kraftwerk und bei der Verteilung bzw. Speicherung, z. B. durch Pumpspeicherwerke, ein.\n2. Die länder- und regionsspezifischen Technologiestandards sowie die Erzeugung in Elektrizitätskraftwerken und/oder in speziellen Kraftwerken mit Kraft-Wärme-Kopplung (KWK) sind berücksichtigt. \n3. Die länderspezifische Energieträgerbereitstellung (mit Anteil der Importe und/oder Eigenversorgung) einschließlich der Eigenschaften der Energieträger (z. B. Elementarzusammensetzung und Heizwert) werden berücksichtigt. \n4. Die Erschließung, Förderung, Verarbeitung und Transportprozesse werden entsprechend der Situation im jeweiligen Stromerzeugerland modelliert. Die unterschiedlichen Produktions- und Verarbeitungsverfahren (Emissionen und Wirkungsgrade) in den verschiedenen Energieerzeugerländern werden einbezogen, z. B. Rohöl-Fördertechnologien oder Abfackel-Raten an den Ölplattformen.\nThermische Energie, Prozessdampf: Die Erzeugung von Dampf und thermischer Energie in Heizkraftwerken wird entsprechend der landesspezifischen Situation (Emissionsgrenzwerte, Energieträgerbasis) modelliert. Der Wirkungsgrad für die thermische Energieerzeugung beträgt per Definition 100% des Energieträgereinsatzes. Für Prozessdampf liegt der Wirkungsgrad bei 85%, 90% und 95%. Die zur Erzeugung von thermischer Energie und Prozessdampf verwendeten Energieträger werden entsprechend der nationalen Situation modelliert (siehe Kapitel Strom oben).\nTransporte: Alle relevanten und bekannten Transportprozesse in Form von See- und Binnenschiffsverkehr sowie Bahn-, Lkw- und der Pipeline-Transport sind enthalten.\nEnergieträger: Die Energieträger werden entsprechend der spezifischen Bereitstellung modelliert (siehe Kapitel Strom oben). \nRaffinerieprodukte: Diesel, Benzin, technische Gase, Heizöl, Schmierstoffe und Rückstände, wie Bitumen, werden mit einem parametrisierten länderspezifischen Raffineriemodell abgebildet. Das Raffinerie-Modell bezieht die länderspezifischen Raffinerie-Technologien (z. B. Emissionsgrenzwerte, interner Energiebedarf etc.) und das länderspezifische Produktspektrum ein, das sich von Land zu Land stark unterscheiden kann. Die Rohöl-Bereitstellung wird gemäß der länderspezifischen Situation mit den jeweiligen ressourcen-spezifischen Eigenschaften modelliert.", "lang": "de"}], "technologicalApplicability": [{"value": "Supply of 1 kWh low voltage (<1kV) electricity to final consumers.", "lang": "en"}, {"value": "Dieses Produkt kann im Baubereich verwendet werden.", "lang": "de"}], "referenceToTechnologyPictogramme": {"shortDescription": [{"value": "energy_electricity_modelling_of_electricity_consumption_mixes.jpg", "lang": "en"}], "type": "source data set", "refObjectId": "e181173d-ea44-4184-94c7-e95f92c5dc7b", "version": "24.01.000", "uri": "../sources/e181173d-ea44-4184-94c7-e95f92c5dc7b.xml"}, "referenceToTechnologyFlowDiagrammOrPicture": [{"shortDescription": [{"value": "energy_electricity_grid_mix_ef_de.jpg", "lang": "en"}], "type": "source data set", "refObjectId": "8cb9e432-b1b8-4e0d-94d3-a68ed982d4d4", "version": "24.01.000", "uri": "../sources/8cb9e432-b1b8-4e0d-94d3-a68ed982d4d4.xml"}, {"shortDescription": [{"value": "energy_electricity_mix_de_2018.jpg", "lang": "en"}], "type": "source data set", "refObjectId": "bfd4b251-1990-4633-b704-5ccd2b9e0e0b", "version": "24.01.000", "uri": "../sources/bfd4b251-1990-4633-b704-5ccd2b9e0e0b.xml"}]}}, "modellingAndValidation": {"LCIMethodAndAllocation": {"typeOfDataSet": "EPD", "other": {"anies": [{"name": "subType", "value": "generic dataset"}]}}, "dataSourcesTreatmentAndRepresentativeness": {"referenceToDataSource": [{"shortDescription": [{"value": "K.Weissermel, H.- J. Arpe: Industrial organic chemistry", "lang": "en"}], "type": "source data set", "refObjectId": "6de1e618-4960-4b0e-aa2c-7f561a1b6f03", "version": "24.01.000", "uri": "../sources/6de1e618-4960-4b0e-aa2c-7f561a1b6f03.xml"}, {"shortDescription": [{"value": "Copper development association: Overview of Recycled Copper", "lang": "en"}], "type": "source data set", "refObjectId": "2b041bb8-adea-4fab-9e28-8abfe409033a", "version": "24.01.000", "uri": "../sources/2b041bb8-adea-4fab-9e28-8abfe409033a.xml"}, {"shortDescription": [{"value": "Smelter Tech: The Reverberatory Furnace ", "lang": "en"}], "type": "source data set", "refObjectId": "b2012fa6-b2f7-4151-b781-aadfaacf4136", "version": "24.01.000", "uri": "../sources/b2012fa6-b2f7-4151-b781-aadfaacf4136.xml"}, {"shortDescription": [{"value": "Process for the production of a plasticized polyvinyl butyral for gluing a base onto a glazing", "lang": "en"}], "type": "source data set", "refObjectId": "9b8971e3-b693-49f0-a0ef-2353e4cfb60b", "version": "24.01.000", "uri": "../sources/9b8971e3-b693-49f0-a0ef-2353e4cfb60b.xml"}, {"shortDescription": [{"value": "LookChem: Manufacture of 1.12-Dodecanedioic Acid", "lang": "en"}], "type": "source data set", "refObjectId": "2ea4220d-0ba7-4351-b99b-545de2232365", "version": "24.01.000", "uri": "../sources/2ea4220d-0ba7-4351-b99b-545de2232365.xml"}, {"shortDescription": [{"value": "Methods of making cyclododecatriene and", "lang": "en"}], "type": "source data set", "refObjectId": "4a1fd634-a5ff-4bd1-a08e-95750cda3a35", "version": "24.01.000", "uri": "../sources/4a1fd634-a5ff-4bd1-a08e-95750cda3a35.xml"}, {"shortDescription": [{"value": "EPA - Health and Environmental Effects Profile for 2-Chloro-1,3-Butadiene, 1984", "lang": "en"}], "type": "source data set", "refObjectId": "56c9aae6-4e0b-4b66-b898-d59cc485198b", "version": "24.01.000", "uri": "../sources/56c9aae6-4e0b-4b66-b898-d59cc485198b.xml"}, {"shortDescription": [{"value": "Chlorpropanes, Chlorobutanes, and Chlorobutenes: Chapter in Ullmann's, 2011", "lang": "en"}], "type": "source data set", "refObjectId": "7e35dd34-81c9-488b-9a69-2b525bfe2999", "version": "24.01.000", "uri": "../sources/7e35dd34-81c9-488b-9a69-2b525bfe2999.xml"}, {"shortDescription": [{"value": "Chloroprene  - Données technico-économiques sur les substances chimiques en France - 2006", "lang": "en"}], "type": "source data set", "refObjectId": "d54f049a-2ece-4140-ac8d-caa694d1d1e9", "version": "24.01.000", "uri": "../sources/d54f049a-2ece-4140-ac8d-caa694d1d1e9.xml"}, {"shortDescription": [{"value": "Renewables Information 2011", "lang": "en"}], "type": "source data set", "refObjectId": "47b981ff-8e4a-4973-8aab-d88611ff3a06", "version": "24.01.000", "uri": "../sources/47b981ff-8e4a-4973-8aab-d88611ff3a06.xml"}, {"shortDescription": [{"value": "eGrid2012 Version 1.0", "lang": "en"}], "type": "source data set", "refObjectId": "3ebd4e78-289a-4b3a-ba90-1071b2ea1a3e", "version": "24.01.000", "uri": "../sources/3ebd4e78-289a-4b3a-ba90-1071b2ea1a3e.xml"}, {"shortDescription": [{"value": "Update of the Environmental Indicators and Energy Payback Time of CIS Modules in Europe, 2010", "lang": "en"}], "type": "source data set", "refObjectId": "acb3a6c1-d206-46ed-8b68-1067eb388a90", "version": "24.01.000", "uri": "../sources/acb3a6c1-d206-46ed-8b68-1067eb388a90.xml"}, {"shortDescription": [{"value": "Sustainability Evaluation of Solar Energy Systems: LCA Analysis (LCA of Thin Film Technologies)", "lang": "en"}], "type": "source data set", "refObjectId": "e831a684-0b46-4c3a-b754-009dd58883ae", "version": "24.01.000", "uri": "../sources/e831a684-0b46-4c3a-b754-009dd58883ae.xml"}, {"shortDescription": [{"value": "Life Cycle Inventories and Life Cycle Assessments of Photovoltaic Systems, 2011", "lang": "en"}], "type": "source data set", "refObjectId": "58b86392-5559-43b1-9d76-7e7a33134051", "version": "24.01.000", "uri": "../sources/58b86392-5559-43b1-9d76-7e7a33134051.xml"}, {"shortDescription": [{"value": "Environmental Life Cycle Inventory of Crystalline Silicon Photovoltaic System Production, 2006", "lang": "en"}], "type": "source data set", "refObjectId": "6b29835e-9afe-410d-a650-c8eb7cedf7a3", "version": "24.01.000", "uri": "../sources/6b29835e-9afe-410d-a650-c8eb7cedf7a3.xml"}, {"shortDescription": [{"value": "Update of environmental indicators and energy payback time of CdTe PV systems in Europe, 2011", "lang": "en"}], "type": "source data set", "refObjectId": "41603ac1-427a-4b74-a6d2-07124c811a06", "version": "24.01.000", "uri": "../sources/41603ac1-427a-4b74-a6d2-07124c811a06.xml"}, {"shortDescription": [{"value": "Energy payback, life cycle CO2 emissions of the BOS in optimized 3.5 MW PV installation", "lang": "en"}], "type": "source data set", "refObjectId": "db43ce49-69ff-436b-b2ba-0d711ee292d2", "version": "24.01.000", "uri": "../sources/db43ce49-69ff-436b-b2ba-0d711ee292d2.xml"}, {"shortDescription": [{"value": "Methodology Guidelines on Life Cycle Assessment of Photovoltaic Electricity, 2009", "lang": "en"}], "type": "source data set", "refObjectId": "83c23f89-16d9-4687-9fb5-b46e5632c594", "version": "24.01.000", "uri": "../sources/83c23f89-16d9-4687-9fb5-b46e5632c594.xml"}, {"shortDescription": [{"value": "Annual European Union greenhouse gas inventory 1990 - 2008 and inventory report 2010", "lang": "en"}], "type": "source data set", "refObjectId": "d19e0017-9ce6-41f6-80d8-1ddcba714d92", "version": "24.01.000", "uri": "../sources/d19e0017-9ce6-41f6-80d8-1ddcba714d92.xml"}, {"shortDescription": [{"value": "Air pollutant emissions in Finland 1990-2008 Informative Inventory report", "lang": "en"}], "type": "source data set", "refObjectId": "4d0b4cd8-ef1e-4b9f-9cc0-a15164f1f1c6", "version": "24.01.000", "uri": "../sources/4d0b4cd8-ef1e-4b9f-9cc0-a15164f1f1c6.xml"}, {"shortDescription": [{"value": "Air pollutant emissions from stationary installations using bioenergy in the NLs BOLK Phase 2", "lang": "en"}], "type": "source data set", "refObjectId": "63ab79ca-79b8-480a-93ff-23b6e10f3301", "version": "24.01.000", "uri": "../sources/63ab79ca-79b8-480a-93ff-23b6e10f3301.xml"}, {"shortDescription": [{"value": "2da Comunicacion Nacional de la Republica Argentina", "lang": "en"}], "type": "source data set", "refObjectId": "4d9277ae-6882-4704-9da8-d864fe7035a6", "version": "24.01.000", "uri": "../sources/4d9277ae-6882-4704-9da8-d864fe7035a6.xml"}, {"shortDescription": [{"value": "2006 IPCC Guidelines for National Greenhouse Gas Inventories", "lang": "en"}], "type": "source data set", "refObjectId": "676b2a43-4d64-47d3-939d-17361afd74df", "version": "24.01.000", "uri": "../sources/676b2a43-4d64-47d3-939d-17361afd74df.xml"}, {"shortDescription": [{"value": "13. Verordnung zur Durchführung des Bundes-Immissionsschutzgesetzes", "lang": "en"}], "type": "source data set", "refObjectId": "d2743393-5fbd-11db-b0de-0800200c9a66", "version": "24.01.000", "uri": "../sources/d2743393-5fbd-11db-b0de-0800200c9a66.xml"}, {"shortDescription": [{"value": "Auswertung PV-Leistung", "lang": "en"}], "type": "source data set", "refObjectId": "fdf1a71b-fde9-4939-b14e-164ff0f4d094", "version": "24.01.000", "uri": "../sources/fdf1a71b-fde9-4939-b14e-164ff0f4d094.xml"}, {"shortDescription": [{"value": "Austria's National Inventory Report 2010", "lang": "en"}], "type": "source data set", "refObjectId": "c175a776-a82f-4739-a0cf-1ac02966df7a", "version": "24.01.000", "uri": "../sources/c175a776-a82f-4739-a0cf-1ac02966df7a.xml"}, {"shortDescription": [{"value": "Austria's Informative Inventory Report (IIR) 2010", "lang": "en"}], "type": "source data set", "refObjectId": "1f692183-8c45-4d9a-87d0-2cb0cdadaf9c", "version": "24.01.000", "uri": "../sources/1f692183-8c45-4d9a-87d0-2cb0cdadaf9c.xml"}, {"shortDescription": [{"value": "Australian National Greenhouse Accounts (NIR)", "lang": "en"}], "type": "source data set", "refObjectId": "6b02aa13-02c4-4f89-b418-51c46249cd74", "version": "24.01.000", "uri": "../sources/6b02aa13-02c4-4f89-b418-51c46249cd74.xml"}, {"shortDescription": [{"value": "Australian electricity generation report 2008", "lang": "en"}], "type": "source data set", "refObjectId": "13f3c0d9-2cd1-40d6-a887-8132d168ce49", "version": "24.01.000", "uri": "../sources/13f3c0d9-2cd1-40d6-a887-8132d168ce49.xml"}, {"shortDescription": [{"value": "Appendix H: Calorific Value, Price, and Emission Coefficients of Energy Kinds", "lang": "en"}], "type": "source data set", "refObjectId": "af10f2b3-4618-47f0-bae4-57e2ba035a5b", "version": "24.01.000", "uri": "../sources/af10f2b3-4618-47f0-bae4-57e2ba035a5b.xml"}, {"shortDescription": [{"value": "Appendix 17 Thermal values and Emission factors energy.xls GWP conversion factors 2006", "lang": "en"}], "type": "source data set", "refObjectId": "b61ddd50-66c1-4b57-a62b-1b3eff1d5c88", "version": "24.01.000", "uri": "../sources/b61ddd50-66c1-4b57-a62b-1b3eff1d5c88.xml"}, {"shortDescription": [{"value": "Anthropogenic Emissions from Energy Activities in India", "lang": "en"}], "type": "source data set", "refObjectId": "074971c8-93ee-41ec-b368-d04410a29499", "version": "24.01.000", "uri": "../sources/074971c8-93ee-41ec-b368-d04410a29499.xml"}, {"shortDescription": [{"value": "Emission Estimation Technique Manual for Fossil Fuel Electric Power Generation Version 2.3", "lang": "en"}], "type": "source data set", "refObjectId": "45ebaf6b-1827-40ab-afc8-5cdf4adbe55f", "version": "24.01.000", "uri": "../sources/45ebaf6b-1827-40ab-afc8-5cdf4adbe55f.xml"}, {"shortDescription": [{"value": "Emisiones atmosféricas de las centrales eléctricas en América del Norte", "lang": "en"}], "type": "source data set", "refObjectId": "c400ff58-c292-41cf-9b9b-2ae4efe728be", "version": "24.01.000", "uri": "../sources/c400ff58-c292-41cf-9b9b-2ae4efe728be.xml"}, {"shortDescription": [{"value": "EMEP/EEA air pollutant emission inventory guidebook - 2009", "lang": "en"}], "type": "source data set", "refObjectId": "9049ae1c-8dc6-4452-bdda-9a0fd0dabef6", "version": "24.01.000", "uri": "../sources/9049ae1c-8dc6-4452-bdda-9a0fd0dabef6.xml"}, {"shortDescription": [{"value": "EMEP/CORINAIR  Emission Inventory Guidebook - 2006", "lang": "en"}], "type": "source data set", "refObjectId": "ed37667c-d18a-4745-bdc3-2d1907a758c5", "version": "24.01.000", "uri": "../sources/ed37667c-d18a-4745-bdc3-2d1907a758c5.xml"}, {"shortDescription": [{"value": "Electricity Gas Australia", "lang": "en"}], "type": "source data set", "refObjectId": "09f34c8b-3240-4a63-ab33-1aca513c5b0a", "version": "24.01.000", "uri": "../sources/09f34c8b-3240-4a63-ab33-1aca513c5b0a.xml"}, {"shortDescription": [{"value": "Electric Power Industry 2009: Year in Review", "lang": "en"}], "type": "source data set", "refObjectId": "8b23bb67-fbe3-48e4-9191-bdb52c8fbb28", "version": "24.01.000", "uri": "../sources/8b23bb67-fbe3-48e4-9191-bdb52c8fbb28.xml"}, {"shortDescription": [{"value": "Directive 2009/28/EC of the European Parliament and of the Council of 23 April 2009", "lang": "en"}], "type": "source data set", "refObjectId": "f3323ac4-38f6-4bff-95b9-0cc97275e91e", "version": "24.01.000", "uri": "../sources/f3323ac4-38f6-4bff-95b9-0cc97275e91e.xml"}, {"shortDescription": [{"value": "Digest of United Kingdom Energy Statistics 2010", "lang": "en"}], "type": "source data set", "refObjectId": "c524c263-6f87-41a1-9998-10806f915e4f", "version": "24.01.000", "uri": "../sources/c524c263-6f87-41a1-9998-10806f915e4f.xml"}, {"shortDescription": [{"value": "Denmark's National Inventory report 2010", "lang": "en"}], "type": "source data set", "refObjectId": "95fbb395-92f4-4993-b88d-5a4cd3ff5471", "version": "24.01.000", "uri": "../sources/95fbb395-92f4-4993-b88d-5a4cd3ff5471.xml"}, {"shortDescription": [{"value": "Danish Emission inventories for stationary combustion plants", "lang": "en"}], "type": "source data set", "refObjectId": "3b917ad4-fb71-43b1-be0b-806537efbfeb", "version": "24.01.000", "uri": "../sources/3b917ad4-fb71-43b1-be0b-806537efbfeb.xml"}, {"shortDescription": [{"value": "Compilation of Air Pollutant Emission Factors", "lang": "en"}], "type": "source data set", "refObjectId": "02564626-8de7-43b0-b671-8dfa43044be8", "version": "24.01.000", "uri": "../sources/02564626-8de7-43b0-b671-8dfa43044be8.xml"}, {"shortDescription": [{"value": "Climate change - Immision Inventory", "lang": "en"}], "type": "source data set", "refObjectId": "5f5d9711-aa38-4ca5-9c43-0b6737d7c48b", "version": "24.01.000", "uri": "../sources/5f5d9711-aa38-4ca5-9c43-0b6737d7c48b.xml"}, {"shortDescription": [{"value": "BVT - Festlegung in ausgewählten industriellen Bereichen als Beitrag zur Erfüllung der Klimasch...", "lang": "en"}], "type": "source data set", "refObjectId": "d7d8f94e-c30b-47f4-aadb-b64a0134cc33", "version": "24.01.000", "uri": "../sources/d7d8f94e-c30b-47f4-aadb-b64a0134cc33.xml"}, {"shortDescription": [{"value": "Brennstoffe und Verbrennungsrechnung, 2. Auflage", "lang": "en"}], "type": "source data set", "refObjectId": "a719ff4c-3b16-4090-b9bc-aac600d7a690", "version": "24.01.000", "uri": "../sources/a719ff4c-3b16-4090-b9bc-aac600d7a690.xml"}, {"shortDescription": [{"value": "Brennstoffe und Verbrennungsrechnung", "lang": "en"}], "type": "source data set", "refObjectId": "cf5a4784-0372-43d0-a814-a2b52132ff11", "version": "24.01.000", "uri": "../sources/cf5a4784-0372-43d0-a814-a2b52132ff11.xml"}, {"shortDescription": [{"value": "Belgium's Greenhouse Gas Inventory (1990-2008)", "lang": "en"}], "type": "source data set", "refObjectId": "14a1e369-d2e8-4054-a4c9-c20f14be6195", "version": "24.01.000", "uri": "../sources/14a1e369-d2e8-4054-a4c9-c20f14be6195.xml"}, {"shortDescription": [{"value": "Greenhouse Gas Emissions in the Netherlands 1990-2008", "lang": "en"}], "type": "source data set", "refObjectId": "a5806d02-3a7d-4ebc-9edb-d82d4a254625", "version": "24.01.000", "uri": "../sources/a5806d02-3a7d-4ebc-9edb-d82d4a254625.xml"}, {"shortDescription": [{"value": "Greenhouse Gas Emissions in Finland 1990-2008", "lang": "en"}], "type": "source data set", "refObjectId": "952089a6-fdba-406f-ac7f-c0c3b2286a65", "version": "24.01.000", "uri": "../sources/952089a6-fdba-406f-ac7f-c0c3b2286a65.xml"}, {"shortDescription": [{"value": "Greenhouse Gas Emissions in Estonia 1990-2008", "lang": "en"}], "type": "source data set", "refObjectId": "d83bb703-1ab5-4306-b324-c6b61e0951a7", "version": "24.01.000", "uri": "../sources/d83bb703-1ab5-4306-b324-c6b61e0951a7.xml"}, {"shortDescription": [{"value": "Greenhouse Gas Emission in Estonia", "lang": "en"}], "type": "source data set", "refObjectId": "a2bb6096-1c77-46a8-8fe5-59b1b3590c83", "version": "24.01.000", "uri": "../sources/a2bb6096-1c77-46a8-8fe5-59b1b3590c83.xml"}, {"shortDescription": [{"value": "GHG Inventories 2008 - Common Reporting Format (CRF)", "lang": "en"}], "type": "source data set", "refObjectId": "cd6f1cfc-f0f8-4270-aa6d-69bdec0e8a7d", "version": "24.01.000", "uri": "../sources/cd6f1cfc-f0f8-4270-aa6d-69bdec0e8a7d.xml"}, {"shortDescription": [{"value": "Full fuel cycle greenhouse gas emission analysis for proposed Kwinana CCGT power station", "lang": "en"}], "type": "source data set", "refObjectId": "4cf7f11b-29ea-482a-acc2-9014aef4e870", "version": "24.01.000", "uri": "../sources/4cf7f11b-29ea-482a-acc2-9014aef4e870.xml"}, {"shortDescription": [{"value": "Ermittlung und Evaluierung von Emissionsfaktoren für Feuerungsanlagen in Deutschland", "lang": "en"}], "type": "source data set", "refObjectId": "580c3724-d564-4c28-bacd-297a8a10ef60", "version": "24.01.000", "uri": "../sources/580c3724-d564-4c28-bacd-297a8a10ef60.xml"}, {"shortDescription": [{"value": "Erarbeitung der Grundlagen für das BVT - Merkblatt Großfeuerungsanlagen", "lang": "en"}], "type": "source data set", "refObjectId": "8f9004d8-69bc-4bfb-ae2c-ec49304abc8d", "version": "24.01.000", "uri": "../sources/8f9004d8-69bc-4bfb-ae2c-ec49304abc8d.xml"}, {"shortDescription": [{"value": "Environmental Report 2008", "lang": "en"}], "type": "source data set", "refObjectId": "010e303b-7e52-4a01-b176-4ac26f4b7eac", "version": "24.01.000", "uri": "../sources/010e303b-7e52-4a01-b176-4ac26f4b7eac.xml"}, {"shortDescription": [{"value": "Energy Statistics  Imports Electricity", "lang": "en"}], "type": "source data set", "refObjectId": "debe5c14-a3c5-4ae1-8f00-ac91dbdcc12d", "version": "24.01.000", "uri": "../sources/debe5c14-a3c5-4ae1-8f00-ac91dbdcc12d.xml"}, {"shortDescription": [{"value": "Energy Futures and Urban Air Pollution: Challenges for China and the United States", "lang": "en"}], "type": "source data set", "refObjectId": "39c74932-1b36-41ed-9ed7-2e8fc678b95a", "version": "24.01.000", "uri": "../sources/39c74932-1b36-41ed-9ed7-2e8fc678b95a.xml"}, {"shortDescription": [{"value": "Energy Consumption, Energy Savings and Emission Analysis for Industrial Motors", "lang": "en"}], "type": "source data set", "refObjectId": "6961baea-190f-4bc4-9aed-c7231f20f128", "version": "24.01.000", "uri": "../sources/6961baea-190f-4bc4-9aed-c7231f20f128.xml"}, {"shortDescription": [{"value": "Emissoes dos Gases Geradores do Efeito Estufa por Termelctricas no Periodo 2000 a 2020", "lang": "en"}], "type": "source data set", "refObjectId": "1a433db5-054d-4795-adc2-1618b790eca2", "version": "24.01.000", "uri": "../sources/1a433db5-054d-4795-adc2-1618b790eca2.xml"}, {"shortDescription": [{"value": "Emissionsschätzungen für SO2, NO2, NMVOC und NH3 in Deutschland 2000-2020", "lang": "en"}], "type": "source data set", "refObjectId": "78626e1d-4507-4562-8c0d-18d84f8bcfe4", "version": "24.01.000", "uri": "../sources/78626e1d-4507-4562-8c0d-18d84f8bcfe4.xml"}, {"shortDescription": [{"value": "Emissionsfaktoren und Kohlenstoffgehalte", "lang": "en"}], "type": "source data set", "refObjectId": "a648a855-48d6-4dfa-a65f-7ef376c077b0", "version": "24.01.000", "uri": "../sources/a648a855-48d6-4dfa-a65f-7ef376c077b0.xml"}, {"shortDescription": [{"value": "Emissions of greenhouse gases in Iceland from 1990 to 2008", "lang": "en"}], "type": "source data set", "refObjectId": "4300d477-7d2e-46ed-bcc4-226e1877565c", "version": "24.01.000", "uri": "../sources/4300d477-7d2e-46ed-bcc4-226e1877565c.xml"}, {"shortDescription": [{"value": "Evaluation Criteria Investment Proposals (translated from hellenic)", "lang": "en"}], "type": "source data set", "refObjectId": "37800c0d-0dbc-436e-99eb-d3790e3c8d1c", "version": "24.01.000", "uri": "../sources/37800c0d-0dbc-436e-99eb-d3790e3c8d1c.xml"}, {"shortDescription": [{"value": "Greenhouse Gas Emissions Inventory Reports of Spain 1990-2008", "lang": "en"}], "type": "source data set", "refObjectId": "308acd86-30a4-42c9-b68c-6ed6a2931877", "version": "24.01.000", "uri": "../sources/308acd86-30a4-42c9-b68c-6ed6a2931877.xml"}, {"shortDescription": [{"value": "Life Cycle Inventory for Electricity Generation in China", "lang": "en"}], "type": "source data set", "refObjectId": "4560b4c3-bf00-470f-b5ed-140cc4d5a3e7", "version": "24.01.000", "uri": "../sources/4560b4c3-bf00-470f-b5ed-140cc4d5a3e7.xml"}, {"shortDescription": [{"value": "Liechtenstein`s Greenhouse Gas Inventory Report 1990 -2008", "lang": "en"}], "type": "source data set", "refObjectId": "d1047ccd-64b4-4f5e-b403-1887547c55d2", "version": "24.01.000", "uri": "../sources/d1047ccd-64b4-4f5e-b403-1887547c55d2.xml"}, {"shortDescription": [{"value": "Latvia's Informative Inventory 1990- 2008", "lang": "en"}], "type": "source data set", "refObjectId": "2ce438a9-0284-4c06-aaab-9cd27962125d", "version": "24.01.000", "uri": "../sources/2ce438a9-0284-4c06-aaab-9cd27962125d.xml"}, {"shortDescription": [{"value": "Italian Greenhouse Gas Inventory 1990-2008", "lang": "en"}], "type": "source data set", "refObjectId": "7a9db98c-5b25-49b9-ace6-ea693b1e1f6d", "version": "24.01.000", "uri": "../sources/7a9db98c-5b25-49b9-ace6-ea693b1e1f6d.xml"}, {"shortDescription": [{"value": "Ireland - Informative Inventory Report 2010", "lang": "en"}], "type": "source data set", "refObjectId": "20b6f41e-6725-4deb-8d68-dd5cd3447cc0", "version": "24.01.000", "uri": "../sources/20b6f41e-6725-4deb-8d68-dd5cd3447cc0.xml"}, {"shortDescription": [{"value": "Inventory of the U.S. Greenhouse Gas Emissions and Sinks (1990 -2008)", "lang": "en"}], "type": "source data set", "refObjectId": "0508ea86-19b8-4557-ad52-10bc9f73452f", "version": "24.01.000", "uri": "../sources/0508ea86-19b8-4557-ad52-10bc9f73452f.xml"}, {"shortDescription": [{"value": "Inventaire des emissions des grandes installations de combustion en France", "lang": "en"}], "type": "source data set", "refObjectId": "72d46923-91d3-4d2e-8565-0c4be7e8f543", "version": "24.01.000", "uri": "../sources/72d46923-91d3-4d2e-8565-0c4be7e8f543.xml"}, {"shortDescription": [{"value": "Integrated Report 2010", "lang": "en"}], "type": "source data set", "refObjectId": "f99161e2-1e5e-4d6a-8c9a-4164b8ee87b5", "version": "24.01.000", "uri": "../sources/f99161e2-1e5e-4d6a-8c9a-4164b8ee87b5.xml"}, {"shortDescription": [{"value": "Integrated Pollution Prevention and Control (IPPC) - Ref. Doc. on the BAT for Large Combustion Plant", "lang": "en"}], "type": "source data set", "refObjectId": "1a8ea509-dbfd-4ba5-805c-e9ba64d6b0cb", "version": "24.01.000", "uri": "../sources/1a8ea509-dbfd-4ba5-805c-e9ba64d6b0cb.xml"}, {"shortDescription": [{"value": "Integrated Pollution Prevention and Control", "lang": "en"}], "type": "source data set", "refObjectId": "e2e153a9-0d09-4447-a398-f9995717eee9", "version": "24.01.000", "uri": "../sources/e2e153a9-0d09-4447-a398-f9995717eee9.xml"}, {"shortDescription": [{"value": "Informative Inventory Report", "lang": "en"}], "type": "source data set", "refObjectId": "6e2d42b4-545d-4450-b5c4-0963dc5a2e59", "version": "24.01.000", "uri": "../sources/6e2d42b4-545d-4450-b5c4-0963dc5a2e59.xml"}, {"shortDescription": [{"value": "India's Initial National Communication to the United Nations Framework Convention on Climate Change", "lang": "en"}], "type": "source data set", "refObjectId": "8ddabeaf-59ca-45e0-b661-5c29be4427f6", "version": "24.01.000", "uri": "../sources/8ddabeaf-59ca-45e0-b661-5c29be4427f6.xml"}, {"shortDescription": [{"value": "Organisation et methodes des inventaires nationaux des emission atmospheriques en France", "lang": "en"}], "type": "source data set", "refObjectId": "1a1829ef-6948-485d-b545-3b72db17264c", "version": "24.01.000", "uri": "../sources/1a1829ef-6948-485d-b545-3b72db17264c.xml"}, {"shortDescription": [{"value": "NIR pour la France au titre de la convention cadre des Nations Unies sur les changements climatiques", "lang": "en"}], "type": "source data set", "refObjectId": "bbc58da8-15bb-4025-90dc-64ae4caed98f", "version": "24.01.000", "uri": "../sources/bbc58da8-15bb-4025-90dc-64ae4caed98f.xml"}, {"shortDescription": [{"value": "New Zealand's Greenhouse Gas Inventory 1990 - 2007", "lang": "en"}], "type": "source data set", "refObjectId": "516c7b37-100e-4481-9f93-00ed916d4541", "version": "24.01.000", "uri": "../sources/516c7b37-100e-4481-9f93-00ed916d4541.xml"}, {"shortDescription": [{"value": "National Inventory Report for 1985-2008 - Hungary", "lang": "en"}], "type": "source data set", "refObjectId": "ccdc8729-d723-4a89-a1a2-60b6cab0c0bb", "version": "24.01.000", "uri": "../sources/ccdc8729-d723-4a89-a1a2-60b6cab0c0bb.xml"}, {"shortDescription": [{"value": "National Inventory Report 2010 Sweden", "lang": "en"}], "type": "source data set", "refObjectId": "15b19a42-6441-4394-bcda-2e49ff1e0fd4", "version": "24.01.000", "uri": "../sources/15b19a42-6441-4394-bcda-2e49ff1e0fd4.xml"}, {"shortDescription": [{"value": "National Inventory Report 2010 Norway", "lang": "en"}], "type": "source data set", "refObjectId": "4b36b132-4a68-431c-bc8b-45d2f5f21fab", "version": "24.01.000", "uri": "../sources/4b36b132-4a68-431c-bc8b-45d2f5f21fab.xml"}, {"shortDescription": [{"value": "National Inventory Report 2010 for Greenhouse Gas Emissions", "lang": "en"}], "type": "source data set", "refObjectId": "23897ee3-ae1e-4a7b-85ea-5c8906d89269", "version": "24.01.000", "uri": "../sources/23897ee3-ae1e-4a7b-85ea-5c8906d89269.xml"}, {"shortDescription": [{"value": "National Inventory Report 2010", "lang": "en"}], "type": "source data set", "refObjectId": "95d3a90d-512b-4b85-8458-f6a859a33d5a", "version": "24.01.000", "uri": "../sources/95d3a90d-512b-4b85-8458-f6a859a33d5a.xml"}, {"shortDescription": [{"value": "National Inventory Report 2010", "lang": "en"}], "type": "source data set", "refObjectId": "ab9a284c-a89e-4f6a-b507-60e0c0b5b551", "version": "24.01.000", "uri": "../sources/ab9a284c-a89e-4f6a-b507-60e0c0b5b551.xml"}, {"shortDescription": [{"value": "National Inventory Report", "lang": "en"}], "type": "source data set", "refObjectId": "8892c020-5266-4d9e-828f-cdf47015d2bb", "version": "24.01.000", "uri": "../sources/8892c020-5266-4d9e-828f-cdf47015d2bb.xml"}, {"shortDescription": [{"value": "National Greenhouse Gas Inventory Report of the Czech Republic, NIR", "lang": "en"}], "type": "source data set", "refObjectId": "b73a174c-74ad-4949-ae92-8e6f321c46b2", "version": "24.01.000", "uri": "../sources/b73a174c-74ad-4949-ae92-8e6f321c46b2.xml"}, {"shortDescription": [{"value": "National Greenhouse Gas Inventory Report of Japan", "lang": "en"}], "type": "source data set", "refObjectId": "9eeb0e0e-b628-4562-afb5-ddc20f317972", "version": "24.01.000", "uri": "../sources/9eeb0e0e-b628-4562-afb5-ddc20f317972.xml"}, {"shortDescription": [{"value": "National Greenhouse Gas Emission Inventory Report 2009 of the Republic of Lithuania", "lang": "en"}], "type": "source data set", "refObjectId": "44b3c207-ff56-4f71-9045-165718811601", "version": "24.01.000", "uri": "../sources/44b3c207-ff56-4f71-9045-165718811601.xml"}, {"shortDescription": [{"value": "Luxembourg´s National Inventory Report 2010 (1990 -2008)", "lang": "en"}], "type": "source data set", "refObjectId": "ff68e8d0-7dde-4614-ba27-cf5262b7859c", "version": "24.01.000", "uri": "../sources/ff68e8d0-7dde-4614-ba27-cf5262b7859c.xml"}, {"shortDescription": [{"value": "Lithuanians's Informative Inventory 2008", "lang": "en"}], "type": "source data set", "refObjectId": "68dd4a61-7521-4dfc-91fe-13513bb38ca1", "version": "24.01.000", "uri": "../sources/68dd4a61-7521-4dfc-91fe-13513bb38ca1.xml"}, {"shortDescription": [{"value": "Switzerland's Greenhouse Gas Inventory 1990-2008", "lang": "en"}], "type": "source data set", "refObjectId": "555d4c66-852f-4743-a1f6-5a47a5a7dc23", "version": "24.01.000", "uri": "../sources/555d4c66-852f-4743-a1f6-5a47a5a7dc23.xml"}, {"shortDescription": [{"value": "Sumas Energy 2 Generation Facility Air Quality Issue Summary", "lang": "en"}], "type": "source data set", "refObjectId": "ef9503bc-edf6-4910-8e93-933446348e4f", "version": "24.01.000", "uri": "../sources/ef9503bc-edf6-4910-8e93-933446348e4f.xml"}, {"shortDescription": [{"value": "Submission under the UN Framework Convention on Climate Change and under the Kyoto Protocol 2010", "lang": "en"}], "type": "source data set", "refObjectId": "f711df00-97d3-47c4-b180-5594b3ebe201", "version": "24.01.000", "uri": "../sources/f711df00-97d3-47c4-b180-5594b3ebe201.xml"}, {"shortDescription": [{"value": "Slovenia's National Inventory Report 2010", "lang": "en"}], "type": "source data set", "refObjectId": "975b5607-1824-4b62-b16d-cd44b9427522", "version": "24.01.000", "uri": "../sources/975b5607-1824-4b62-b16d-cd44b9427522.xml"}, {"shortDescription": [{"value": "Slovak Republic National Inventory Report 2010", "lang": "en"}], "type": "source data set", "refObjectId": "7ed2df76-c25a-428b-870f-bb116cc4ba12", "version": "24.01.000", "uri": "../sources/7ed2df76-c25a-428b-870f-bb116cc4ba12.xml"}, {"shortDescription": [{"value": "Romania's Greenhouse Gas Inventory 1989-2008", "lang": "en"}], "type": "source data set", "refObjectId": "648eabe1-6171-481e-9385-0aa23ca08a9a", "version": "24.01.000", "uri": "../sources/648eabe1-6171-481e-9385-0aa23ca08a9a.xml"}, {"shortDescription": [{"value": "Romanian Informative Inventory 2008", "lang": "en"}], "type": "source data set", "refObjectId": "fef1f400-2e11-4dbe-88eb-459269290154", "version": "24.01.000", "uri": "../sources/fef1f400-2e11-4dbe-88eb-459269290154.xml"}, {"shortDescription": [{"value": "Richtlinie 2009/28/EG des Europäischen Parlaments und des Rates vom 23. April 2009", "lang": "en"}], "type": "source data set", "refObjectId": "f494c11e-737c-4b1b-a911-1d511177b5e3", "version": "24.01.000", "uri": "../sources/f494c11e-737c-4b1b-a911-1d511177b5e3.xml"}, {"shortDescription": [{"value": "Renewables 2010", "lang": "en"}], "type": "source data set", "refObjectId": "b431a232-fe5b-41c5-87b0-94fdb402a733", "version": "24.01.000", "uri": "../sources/b431a232-fe5b-41c5-87b0-94fdb402a733.xml"}, {"shortDescription": [{"value": "Power Hungry: Reinventing The U.S. Electric Grid", "lang": "en"}], "type": "source data set", "refObjectId": "e8f646de-4e1f-40ab-8294-46f81ad67fd1", "version": "24.01.000", "uri": "../sources/e8f646de-4e1f-40ab-8294-46f81ad67fd1.xml"}, {"shortDescription": [{"value": "Power Connections: Canadian Electricity Trade and Foreign Policy", "lang": "en"}], "type": "source data set", "refObjectId": "15fec28d-cbbc-42a8-aed9-4140a217c74e", "version": "24.01.000", "uri": "../sources/15fec28d-cbbc-42a8-aed9-4140a217c74e.xml"}, {"shortDescription": [{"value": "Portuguese National Inventory Report on Grennhouse Gases, 1990-2008", "lang": "en"}], "type": "source data set", "refObjectId": "a25eb4da-f802-4e7b-b8f9-5db9d9d59fc2", "version": "24.01.000", "uri": "../sources/a25eb4da-f802-4e7b-b8f9-5db9d9d59fc2.xml"}, {"shortDescription": [{"value": "Portuguese Informative Inventory 1990-2008", "lang": "en"}], "type": "source data set", "refObjectId": "0aadf465-cc80-4843-93aa-1d2fc5a16263", "version": "24.01.000", "uri": "../sources/0aadf465-cc80-4843-93aa-1d2fc5a16263.xml"}, {"shortDescription": [{"value": "Poland's Informative Inventory 2010", "lang": "en"}], "type": "source data set", "refObjectId": "2e7f9df2-2d00-4ed3-a366-001dc03e43db", "version": "24.01.000", "uri": "../sources/2e7f9df2-2d00-4ed3-a366-001dc03e43db.xml"}, {"shortDescription": [{"value": "Verhaltenes Lächeln auf langen Gesichtern", "lang": "en"}], "type": "source data set", "refObjectId": "71fd4cb6-d468-4dca-8b65-b5b35ad6f80c", "version": "24.01.000", "uri": "../sources/71fd4cb6-d468-4dca-8b65-b5b35ad6f80c.xml"}, {"shortDescription": [{"value": "UK Greenhouse gas inventory, 1990 to 2008", "lang": "en"}], "type": "source data set", "refObjectId": "34a298be-4daa-457f-bd8f-075755d1d42d", "version": "24.01.000", "uri": "../sources/34a298be-4daa-457f-bd8f-075755d1d42d.xml"}, {"shortDescription": [{"value": "Turkey Greenhouse gas Inventory, 1990 to 2008", "lang": "en"}], "type": "source data set", "refObjectId": "6c59444d-2cf1-426d-9df7-93e60364c955", "version": "24.01.000", "uri": "../sources/6c59444d-2cf1-426d-9df7-93e60364c955.xml"}, {"shortDescription": [{"value": "The European Pollutant Release and Transfer Register", "lang": "en"}], "type": "source data set", "refObjectId": "68570e54-3d75-4c1f-b88d-df2a66c2ba30", "version": "24.01.000", "uri": "../sources/68570e54-3d75-4c1f-b88d-df2a66c2ba30.xml"}, {"shortDescription": [{"value": "The CEA Mercury program", "lang": "en"}], "type": "source data set", "refObjectId": "3b65ee48-c719-40f4-ab73-7f0383584712", "version": "24.01.000", "uri": "../sources/3b65ee48-c719-40f4-ab73-7f0383584712.xml"}, {"shortDescription": [{"value": "Telefonische Recherche - Preis Kraftwerksnebenprodukte", "lang": "en"}], "type": "source data set", "refObjectId": "cbede9c2-03b5-457c-a947-6e944f9d39fc", "version": "24.01.000", "uri": "../sources/cbede9c2-03b5-457c-a947-6e944f9d39fc.xml"}, {"shortDescription": [{"value": "Plant-by-Plant emissions of SO2, NOx and dust and energy input to large combustion plants covered...", "lang": "en"}], "type": "source data set", "refObjectId": "0f4a3245-3bc0-49ee-8da0-42405554f541", "version": "24.01.000", "uri": "../sources/0f4a3245-3bc0-49ee-8da0-42405554f541.xml"}, {"shortDescription": [{"value": "The European offshore wind industry - key trends and statistics 2014", "lang": "en"}], "type": "source data set", "refObjectId": "f0a58cb7-9486-4458-a6a5-4dbef32d871b", "version": "24.01.000", "uri": "../sources/f0a58cb7-9486-4458-a6a5-4dbef32d871b.xml"}, {"shortDescription": [{"value": "China Electric Power Yearbook 2015", "lang": "en"}], "type": "source data set", "refObjectId": "3875965d-fb85-4dc4-94ef-3372b30d7ef9", "version": "24.01.000", "uri": "../sources/3875965d-fb85-4dc4-94ef-3372b30d7ef9.xml"}, {"shortDescription": [{"value": "Bruttostromerzeugung in Deutschland ab 1990 nach Energieträgern ", "lang": "en"}], "type": "source data set", "refObjectId": "5da9b82b-f76e-43fd-89de-6719d195eee0", "version": "24.01.000", "uri": "../sources/5da9b82b-f76e-43fd-89de-6719d195eee0.xml"}, {"shortDescription": [{"value": "Wind in power 2016 - European statistics  ", "lang": "en"}], "type": "source data set", "refObjectId": "038ede2d-0650-4acf-89c4-623cad30bbb9", "version": "24.01.000", "uri": "../sources/038ede2d-0650-4acf-89c4-623cad30bbb9.xml"}, {"shortDescription": [{"value": "The European offshore wind industry - key trends and statistics 2015", "lang": "en"}], "type": "source data set", "refObjectId": "d5cfdcc8-52ec-4fdb-8180-4150014ed370", "version": "24.01.000", "uri": "../sources/d5cfdcc8-52ec-4fdb-8180-4150014ed370.xml"}, {"shortDescription": [{"value": "IEA Wind - 2016 Annual report   ", "lang": "en"}], "type": "source data set", "refObjectId": "2593f5d7-97c7-415c-8b5e-035d7178abce", "version": "24.01.000", "uri": "../sources/2593f5d7-97c7-415c-8b5e-035d7178abce.xml"}, {"shortDescription": [{"value": "Statistical Yearbook 2015", "lang": "en"}], "type": "source data set", "refObjectId": "888c15fe-6986-4434-a7e2-39f2b06d0d8e", "version": "24.01.000", "uri": "../sources/888c15fe-6986-4434-a7e2-39f2b06d0d8e.xml"}, {"shortDescription": [{"value": "Energy Balances of OECD Countries 2017", "lang": "en"}], "type": "source data set", "refObjectId": "931e99ab-e2b5-4667-bfd6-d8517f702997", "version": "24.01.000", "uri": "../sources/931e99ab-e2b5-4667-bfd6-d8517f702997.xml"}, {"shortDescription": [{"value": "Energy Statistics of OECD Countries 2017", "lang": "en"}], "type": "source data set", "refObjectId": "fc9d620f-c3b9-46b6-a592-099cdede9eca", "version": "24.01.000", "uri": "../sources/fc9d620f-c3b9-46b6-a592-099cdede9eca.xml"}, {"shortDescription": [{"value": "Energy Balances of Non-OECD Countries 2017 ", "lang": "en"}], "type": "source data set", "refObjectId": "cf73d907-7766-432e-84f7-73bde6bd0e18", "version": "24.01.000", "uri": "../sources/cf73d907-7766-432e-84f7-73bde6bd0e18.xml"}, {"shortDescription": [{"value": "Energy Statistics of Non-OECD Countries 2017", "lang": "en"}], "type": "source data set", "refObjectId": "df41463a-39bb-4787-a194-c676ba6f8523", "version": "24.01.000", "uri": "../sources/df41463a-39bb-4787-a194-c676ba6f8523.xml"}, {"shortDescription": [{"value": "World Energy Statistics 2017", "lang": "en"}], "type": "source data set", "refObjectId": "f8733bf1-8713-445d-9f5c-511452ed6e9c", "version": "24.01.000", "uri": "../sources/f8733bf1-8713-445d-9f5c-511452ed6e9c.xml"}, {"shortDescription": [{"value": "Electricity Information 2017", "lang": "en"}], "type": "source data set", "refObjectId": "f3bbd3d5-6143-400c-ba0c-4d36b745ef9d", "version": "24.01.000", "uri": "../sources/f3bbd3d5-6143-400c-ba0c-4d36b745ef9d.xml"}, {"shortDescription": [{"value": "Documentation of data quality management", "lang": "en"}], "type": "source data set", "refObjectId": "e3bd9bbf-2c3c-42aa-8892-fd13f1065ca5", "version": "24.01.000", "uri": "../sources/e3bd9bbf-2c3c-42aa-8892-fd13f1065ca5.xml"}, {"shortDescription": [{"value": "GaBi Database Edition 2021, CUP2021.01", "lang": "en"}], "type": "source data set", "refObjectId": "1cece811-7501-44d4-8067-9259bd5cb835", "version": "00.01.000", "uri": "../sources/1cece811-7501-44d4-8067-9259bd5cb835.xml"}, {"shortDescription": [{"value": "Sphera Managed LCA Content Databases (all versions)", "lang": "en"}], "type": "source data set", "refObjectId": "28d74cc0-db8b-4d7e-bc44-5f6d56ce0c4a", "version": "00.03.002", "uri": "../sources/28d74cc0-db8b-4d7e-bc44-5f6d56ce0c4a.xml"}], "useAdviceForDataSet": [{"value": "Use by low voltage electricity consumers without own electricity transformers (e.g. SME and private households), which use electricity directly from the grid. The data set can be used for all LCA/CF studies where low voltage electricity is needed. Combination with individual unit processes using this commodity enables the generation of user-specific (product) LCAs.", "lang": "en"}, {"value": "Der Datensatz repräsentiert ein Cradle to Gate Inventar. Er kann verwendet werden, um die Lieferkette des jeweiligen Produktes in einer repräsentativen Weise zu charakterisieren. Die Kombination mit einzelnen Einheitenprozessen und diesem Produkt ermöglicht die Erstellung von anwenderspezifischen (Produkt-) LCAs.", "lang": "de"}]}, "validation": {"review": [{"referenceToNameOfReviewerAndInstitution": [{"shortDescription": [{"value": "Sphera Solutions GmbH", "lang": "en"}], "type": "contact data set", "refObjectId": "d7fa0337-f279-430d-becf-7f3111a85010", "version": "24.01.000", "uri": "../contacts/d7fa0337-f279-430d-becf-7f3111a85010.xml"}], "type": "Dependent internal review"}, {"referenceToNameOfReviewerAndInstitution": [{"shortDescription": [{"value": "Sphera Product Sustainability user forum", "lang": "en"}], "type": "contact data set", "refObjectId": "8f1306f0-7b83-4f36-a537-aa83f0498266", "version": "24.01.000", "uri": "../contacts/8f1306f0-7b83-4f36-a537-aa83f0498266.xml"}], "type": "Independent external review"}]}, "complianceDeclarations": {"compliance": [{"referenceToComplianceSystem": {"shortDescription": [{"value": "EN 15804+A2 (EF 3.1)", "lang": "de"}, {"value": "EN 15804+A2 (EF 3.1)", "lang": "en"}], "type": "source data set", "refObjectId": "d4aa3ec7-b1d7-4a4a-a6cb-37af88dcc902", "version": "00.01.000", "uri": "../sources/d4aa3ec7-b1d7-4a4a-a6cb-37af88dcc902.xml"}, "approvalOfOverallCompliance": "Fully compliant"}]}}, "administrativeInformation": {"dataGenerator": {"referenceToPersonOrEntityGeneratingTheDataSet": [{"shortDescription": [{"value": "Sphera Solutions GmbH", "lang": "en"}], "type": "contact data set", "refObjectId": "d7fa0337-f279-430d-becf-7f3111a85010", "version": "24.01.000", "uri": "../contacts/d7fa0337-f279-430d-becf-7f3111a85010.xml"}]}, "dataEntryBy": {"timeStamp": 1718121647000, "referenceToDataSetFormat": [{"shortDescription": [{"value": "ILCD format 1.1", "lang": "de"}, {"value": "ILCD format 1.1", "lang": "en"}], "type": "source data set", "refObjectId": "a97a0155-0234-4b87-b4ce-a45da52f2a40", "version": "01.00.000", "uri": "../sources/a97a0155-0234-4b87-b4ce-a45da52f2a40.xml"}, {"shortDescription": [{"value": "EPD-Datenformaterweiterungen v1.2", "lang": "de"}, {"value": "EPD Data Format Extensions v1.2", "lang": "en"}], "type": "source data set", "refObjectId": "a29449fd-aa2f-4de8-b5d7-4b06b43c6fde", "version": "00.01.000", "uri": "../sources/a29449fd-aa2f-4de8-b5d7-4b06b43c6fde.xml"}], "referenceToPersonOrEntityEnteringTheData": {"shortDescription": [{"value": "Sphera Solutions GmbH", "lang": "en"}], "type": "contact data set", "refObjectId": "d7fa0337-f279-430d-becf-7f3111a85010", "version": "24.01.000", "uri": "../contacts/d7fa0337-f279-430d-becf-7f3111a85010.xml"}}, "publicationAndOwnership": {"dataSetVersion": "20.24.070", "referenceToPrecedingDataSetVersion": [{"shortDescription": [{"value": "Electricity grid mix 2019", "lang": "en"}], "type": "process data set", "refObjectId": "578f004b-57e4-45d4-b0b6-e9ff8b011d81", "uri": "https://www.oekobaudat.de/OEKOBAU.DAT/resource/processes/578f004b-57e4-45d4-b0b6-e9ff8b011d81?version=20.23.050"}], "referenceToRegistrationAuthority": {"shortDescription": [{"value": "Sphera Solutions GmbH", "lang": "en"}], "type": "contact data set", "refObjectId": "d7fa0337-f279-430d-becf-7f3111a85010", "version": "24.01.000", "uri": "../contacts/d7fa0337-f279-430d-becf-7f3111a85010.xml"}, "referenceToOwnershipOfDataSet": {"shortDescription": [{"value": "Sphera Solutions GmbH", "lang": "en"}], "type": "contact data set", "refObjectId": "d7fa0337-f279-430d-becf-7f3111a85010", "version": "24.01.000", "uri": "../contacts/d7fa0337-f279-430d-becf-7f3111a85010.xml"}, "copyright": true, "licenseType": "Free of charge for all users and uses", "accessRestrictions": [{"value": "The license conditions as stated on https://www.oekobaudat.de/apply.", "lang": "en"}, {"value": "Es gelten die Lizenzbedingungen wie sie auf https://www.oekobaudat.de/ genannt sind.", "lang": "de"}], "other": {"anies": [{"name": "referenceToPublisher", "value": {"shortDescription": [{"value": "BBSR", "lang": "en"}], "type": "contact data set", "refObjectId": "f11651e0-7877-11e3-981f-0800200c9a66", "version": "00.01.000", "uri": "../contacts/f11651e0-7877-11e3-981f-0800200c9a66.xml"}}]}}}, "exchanges": {"exchange": [{"dataSetInternalID": 100152, "referenceToFlowDataSet": {"shortDescription": [{"value": "Electricity grid mix 2019", "lang": "en"}, {"value": "Strom für Gebäudebetrieb 2019", "lang": "de"}], "type": "flow data set", "refObjectId": "890a70b7-b677-4e2a-8a1b-7d017e0a10ae", "version": "24.01.000", "uri": "../flows/890a70b7-b677-4e2a-8a1b-7d017e0a10ae.xml"}, "meanAmount": 3.6, "referenceFlow": true, "resultingflowAmount": 3.6, "flowProperties": [{"name": [{"lang": "en", "value": "Net calorific value"}, {"lang": "de", "value": "Unterer Heizwert"}], "uuid": "93a60a56-a3c8-11da-a746-0800200c9a66", "referenceFlowProperty": true, "meanValue": 1.0, "referenceUnit": "MJ", "unitGroupUUID": "93a60a57-a3c8-11da-a746-0800200c9a66"}], "typeOfFlow": "Product flow", "classification": {"classHierarchy": "Valuable substances / Energy carrier / Electric power", "name": "GaBiCategories"}}, {"dataSetInternalID": 100153, "referenceToFlowDataSet": {"shortDescription": [{"value": "Use of renewable primary energy as energy carrier (PERE)", "lang": "en"}, {"value": "Erneuerbare Primärenergie als Energieträger (PERE)", "lang": "de"}], "type": "flow data set", "refObjectId": "20f32be5-0398-4288-9b6d-accddd195317", "version": "24.01.000", "uri": "../flows/20f32be5-0398-4288-9b6d-accddd195317.xml"}, "exchange direction": "INPUT", "other": {"anies": [{"value": "5.72566298156324", "module": "B6"}, {"name": "referenceToUnitGroupDataSet", "value": {"shortDescription": [{"value": "MJ", "lang": "en"}], "type": "unit group data set", "refObjectId": "93a60a57-a3c8-11da-a746-0800200c9a66", "version": "03.00.000", "uri": "../unitgroups/93a60a57-a3c8-11da-a746-0800200c9a66.xml"}}]}, "resolvedFlowVersion": "38.00.000", "flowProperties": [], "typeOfFlow": "Other flow", "classification": {"classHierarchy": "Quantities", "name": "GaBiCategories"}}, {"dataSetInternalID": 100154, "referenceToFlowDataSet": {"shortDescription": [{"value": "Use of renewable primary energy resources used as raw materials (PERM)", "lang": "en"}, {"value": "Erneuerbare Primärenergie zur stofflichen Nutzung (PERM)", "lang": "de"}], "type": "flow data set", "refObjectId": "fb3ec0de-548d-4508-aea5-00b73bf6f702", "version": "24.01.000", "uri": "../flows/fb3ec0de-548d-4508-aea5-00b73bf6f702.xml"}, "exchange direction": "INPUT", "other": {"anies": [{"value": "0", "module": "B6"}, {"name": "referenceToUnitGroupDataSet", "value": {"shortDescription": [{"value": "MJ", "lang": "en"}], "type": "unit group data set", "refObjectId": "93a60a57-a3c8-11da-a746-0800200c9a66", "version": "03.00.000", "uri": "../unitgroups/93a60a57-a3c8-11da-a746-0800200c9a66.xml"}}]}, "resolvedFlowVersion": "38.00.000", "flowProperties": [], "typeOfFlow": "Other flow", "classification": {"classHierarchy": "Quantities", "name": "GaBiCategories"}}, {"dataSetInternalID": 100155, "referenceToFlowDataSet": {"shortDescription": [{"value": "Total use of renewable primary energy (PERT)", "lang": "en"}, {"value": "Total erneuerbare Primärenergie (PERT)", "lang": "de"}], "type": "flow data set", "refObjectId": "53f97275-fa8a-4cdd-9024-65936002acd0", "version": "24.01.000", "uri": "../flows/53f97275-fa8a-4cdd-9024-65936002acd0.xml"}, "exchange direction": "INPUT", "other": {"anies": [{"value": "5.72566298156324", "module": "B6"}, {"name": "referenceToUnitGroupDataSet", "value": {"shortDescription": [{"value": "MJ", "lang": "en"}], "type": "unit group data set", "refObjectId": "93a60a57-a3c8-11da-a746-0800200c9a66", "version": "03.00.000", "uri": "../unitgroups/93a60a57-a3c8-11da-a746-0800200c9a66.xml"}}]}, "resolvedFlowVersion": "38.00.000", "flowProperties": [], "typeOfFlow": "Other flow", "classification": {"classHierarchy": "Quantities / Environmental quantities / EPD EN 15804 / LCI indicators", "name": "GaBiCategories"}}, {"dataSetInternalID": 100156, "referenceToFlowDataSet": {"shortDescription": [{"value": "Use of non renewable primary energy as energy carrier (PENRE)", "lang": "en"}, {"value": "Nicht-erneuerbare Primärenergie als Energieträger (PENRE)", "lang": "de"}], "type": "flow data set", "refObjectId": "ac857178-2b45-46ec-892a-a9a4332f0372", "version": "24.01.000", "uri": "../flows/ac857178-2b45-46ec-892a-a9a4332f0372.xml"}, "exchange direction": "INPUT", "other": {"anies": [{"value": "6.03090101519868", "module": "B6"}, {"name": "referenceToUnitGroupDataSet", "value": {"shortDescription": [{"value": "MJ", "lang": "en"}], "type": "unit group data set", "refObjectId": "93a60a57-a3c8-11da-a746-0800200c9a66", "version": "03.00.000", "uri": "../unitgroups/93a60a57-a3c8-11da-a746-0800200c9a66.xml"}}]}, "resolvedFlowVersion": "38.00.000", "flowProperties": [], "typeOfFlow": "Other flow", "classification": {"classHierarchy": "Quantities", "name": "GaBiCategories"}}, {"dataSetInternalID": 100157, "referenceToFlowDataSet": {"shortDescription": [{"value": "Use of non renewable primary energy resources used as raw materials (PENRM)", "lang": "en"}, {"value": "Nicht-erneuerbare Primärenergie zur stofflichen Nutzung (PENRM)", "lang": "de"}], "type": "flow data set", "refObjectId": "1421caa0-679d-4bf4-b282-0eb850ccae27", "version": "24.01.000", "uri": "../flows/1421caa0-679d-4bf4-b282-0eb850ccae27.xml"}, "exchange direction": "INPUT", "other": {"anies": [{"value": "0", "module": "B6"}, {"name": "referenceToUnitGroupDataSet", "value": {"shortDescription": [{"value": "MJ", "lang": "en"}], "type": "unit group data set", "refObjectId": "93a60a57-a3c8-11da-a746-0800200c9a66", "version": "03.00.000", "uri": "../unitgroups/93a60a57-a3c8-11da-a746-0800200c9a66.xml"}}]}, "resolvedFlowVersion": "38.00.000", "flowProperties": [], "typeOfFlow": "Other flow", "classification": {"classHierarchy": "Quantities", "name": "GaBiCategories"}}, {"dataSetInternalID": 100158, "referenceToFlowDataSet": {"shortDescription": [{"value": "Total use of non renewable primary energy resource (PENRT)", "lang": "en"}, {"value": "Total nicht-erneuerbare Primärenergie (PENRT)", "lang": "de"}], "type": "flow data set", "refObjectId": "06159210-646b-4c8d-8583-da9b3b95a6c1", "version": "24.01.000", "uri": "../flows/06159210-646b-4c8d-8583-da9b3b95a6c1.xml"}, "exchange direction": "INPUT", "other": {"anies": [{"value": "6.03090101519868", "module": "B6"}, {"name": "referenceToUnitGroupDataSet", "value": {"shortDescription": [{"value": "MJ", "lang": "en"}], "type": "unit group data set", "refObjectId": "93a60a57-a3c8-11da-a746-0800200c9a66", "version": "03.00.000", "uri": "../unitgroups/93a60a57-a3c8-11da-a746-0800200c9a66.xml"}}]}, "resolvedFlowVersion": "38.00.000", "flowProperties": [], "typeOfFlow": "Other flow", "classification": {"classHierarchy": "Quantities / Environmental quantities / EPD EN 15804 / LCI indicators", "name": "GaBiCategories"}}, {"dataSetInternalID": 100159, "referenceToFlowDataSet": {"shortDescription": [{"value": "Use of secondary material (SM)", "lang": "en"}, {"value": "Einsatz von Sekundärstoffen (SM)", "lang": "de"}], "type": "flow data set", "refObjectId": "c6a1f35f-2d09-4f54-8dfb-97e502e1ce92", "version": "24.01.000", "uri": "../flows/c6a1f35f-2d09-4f54-8dfb-97e502e1ce92.xml"}, "exchange direction": "INPUT", "other": {"anies": [{"value": "0", "module": "B6"}, {"name": "referenceToUnitGroupDataSet", "value": {"shortDescription": [{"value": "kg", "lang": "en"}], "type": "unit group data set", "refObjectId": "93a60a57-a4c8-11da-a746-0800200c9a66", "version": "03.00.000", "uri": "../unitgroups/93a60a57-a4c8-11da-a746-0800200c9a66.xml"}}]}, "resolvedFlowVersion": "38.00.000", "flowProperties": [], "typeOfFlow": "Other flow", "classification": {"classHierarchy": "Quantities / Environmental quantities / EPD EN 15804 / LCI indicators", "name": "GaBiCategories"}}, {"dataSetInternalID": 100160, "referenceToFlowDataSet": {"shortDescription": [{"value": "Use of renewable secondary fuels (SF)", "lang": "en"}, {"value": "Erneuerbare Sekundärbrennstoffe (SF)", "lang": "de"}], "type": "flow data set", "refObjectId": "64333088-a55f-4aa2-9a31-c10b07816787", "version": "24.01.000", "uri": "../flows/64333088-a55f-4aa2-9a31-c10b07816787.xml"}, "exchange direction": "INPUT", "other": {"anies": [{"value": "0", "module": "B6"}, {"name": "referenceToUnitGroupDataSet", "value": {"shortDescription": [{"value": "MJ", "lang": "en"}], "type": "unit group data set", "refObjectId": "93a60a57-a3c8-11da-a746-0800200c9a66", "version": "03.00.000", "uri": "../unitgroups/93a60a57-a3c8-11da-a746-0800200c9a66.xml"}}]}, "resolvedFlowVersion": "38.00.000", "flowProperties": [], "typeOfFlow": "Other flow", "classification": {"classHierarchy": "Quantities / Environmental quantities / EPD EN 15804 / LCI indicators", "name": "GaBiCategories"}}, {"dataSetInternalID": 100161, "referenceToFlowDataSet": {"shortDescription": [{"value": "Use of non renewable secondary fuels (NRSF)", "lang": "en"}, {"value": "Nicht erneuerbare Sekundärbrennstoffe (NRSF)", "lang": "de"}], "type": "flow data set", "refObjectId": "89def144-d39a-4287-b86f-efde453ddcb2", "version": "24.01.000", "uri": "../flows/89def144-d39a-4287-b86f-efde453ddcb2.xml"}, "exchange direction": "INPUT", "other": {"anies": [{"value": "0", "module": "B6"}, {"name": "referenceToUnitGroupDataSet", "value": {"shortDescription": [{"value": "MJ", "lang": "en"}], "type": "unit group data set", "refObjectId": "93a60a57-a3c8-11da-a746-0800200c9a66", "version": "03.00.000", "uri": "../unitgroups/93a60a57-a3c8-11da-a746-0800200c9a66.xml"}}]}, "resolvedFlowVersion": "38.00.000", "flowProperties": [], "typeOfFlow": "Other flow", "classification": {"classHierarchy": "Quantities / Environmental quantities / EPD EN 15804 / LCI indicators", "name": "GaBiCategories"}}, {"dataSetInternalID": 100162, "referenceToFlowDataSet": {"shortDescription": [{"value": "Net use of fresh water (FW)", "lang": "en"}, {"value": "Nettoeinsatz von Süßwasserressourcen (FW)", "lang": "de"}], "type": "flow data set", "refObjectId": "3cf952c8-f3a4-461d-8c96-96456ca62246", "version": "24.01.000", "uri": "../flows/3cf952c8-f3a4-461d-8c96-96456ca62246.xml"}, "exchange direction": "INPUT", "other": {"anies": [{"value": "0.0019674031960842", "module": "B6"}, {"name": "referenceToUnitGroupDataSet", "value": {"shortDescription": [{"value": "m3", "lang": "en"}], "type": "unit group data set", "refObjectId": "93a60a57-a3c8-12da-a746-0800200c9a66", "version": "03.00.000", "uri": "../unitgroups/93a60a57-a3c8-12da-a746-0800200c9a66.xml"}}]}, "resolvedFlowVersion": "38.00.000", "flowProperties": [], "typeOfFlow": "Other flow", "classification": {"classHierarchy": "Quantities / Environmental quantities / EPD EN 15804 / LCI indicators", "name": "GaBiCategories"}}, {"dataSetInternalID": 100163, "referenceToFlowDataSet": {"shortDescription": [{"value": "Hazardous waste disposed (HWD)", "lang": "en"}, {"value": "Gefährlicher Abfall zur Deponie (HWD)", "lang": "de"}], "type": "flow data set", "refObjectId": "430f9e0f-59b2-46a0-8e0d-55e0e84948fc", "version": "24.01.000", "uri": "../flows/430f9e0f-59b2-46a0-8e0d-55e0e84948fc.xml"}, "exchange direction": "OUTPUT", "other": {"anies": [{"value": "1.31245696758294E-8", "module": "B6"}, {"name": "referenceToUnitGroupDataSet", "value": {"shortDescription": [{"value": "kg", "lang": "en"}], "type": "unit group data set", "refObjectId": "93a60a57-a4c8-11da-a746-0800200c9a66", "version": "03.00.000", "uri": "../unitgroups/93a60a57-a4c8-11da-a746-0800200c9a66.xml"}}]}, "resolvedFlowVersion": "38.00.000", "flowProperties": [], "typeOfFlow": "Other flow", "classification": {"classHierarchy": "Quantities / Environmental quantities / EPD EN 15804 / LCI indicators", "name": "GaBiCategories"}}, {"dataSetInternalID": 100164, "referenceToFlowDataSet": {"shortDescription": [{"value": "Non harzardous waste disposed (NHWD)", "lang": "en"}, {"value": "Entsorgter nicht gefährlicher Abfall (NHWD)", "lang": "de"}], "type": "flow data set", "refObjectId": "b29ef66b-e286-4afa-949f-62f1a7b4d7fa", "version": "24.01.000", "uri": "../flows/b29ef66b-e286-4afa-949f-62f1a7b4d7fa.xml"}, "exchange direction": "OUTPUT", "other": {"anies": [{"value": "0.00559724865446092", "module": "B6"}, {"name": "referenceToUnitGroupDataSet", "value": {"shortDescription": [{"value": "kg", "lang": "en"}], "type": "unit group data set", "refObjectId": "93a60a57-a4c8-11da-a746-0800200c9a66", "version": "03.00.000", "uri": "../unitgroups/93a60a57-a4c8-11da-a746-0800200c9a66.xml"}}]}, "resolvedFlowVersion": "38.00.000", "flowProperties": [], "typeOfFlow": "Other flow", "classification": {"classHierarchy": "Quantities / Environmental quantities / EPD EN 15804 / LCI indicators", "name": "GaBiCategories"}}, {"dataSetInternalID": 100165, "referenceToFlowDataSet": {"shortDescription": [{"value": "Radioactive waste disposed (RWD)", "lang": "en"}, {"value": "Entsorgter radioaktiver Abfall (RWD)", "lang": "de"}], "type": "flow data set", "refObjectId": "3449546e-52ad-4b39-b809-9fb77cea8ff6", "version": "24.01.000", "uri": "../flows/3449546e-52ad-4b39-b809-9fb77cea8ff6.xml"}, "exchange direction": "OUTPUT", "other": {"anies": [{"value": "0.000573629812204406", "module": "B6"}, {"name": "referenceToUnitGroupDataSet", "value": {"shortDescription": [{"value": "kg", "lang": "en"}], "type": "unit group data set", "refObjectId": "93a60a57-a4c8-11da-a746-0800200c9a66", "version": "03.00.000", "uri": "../unitgroups/93a60a57-a4c8-11da-a746-0800200c9a66.xml"}}]}, "resolvedFlowVersion": "38.00.000", "flowProperties": [], "typeOfFlow": "Other flow", "classification": {"classHierarchy": "Quantities / Environmental quantities / EPD EN 15804 / LCI indicators", "name": "GaBiCategories"}}, {"dataSetInternalID": 100166, "referenceToFlowDataSet": {"shortDescription": [{"value": "Components for re-use (CRU)", "lang": "en"}, {"value": "Komponenten für die Wiederverwendung (CRU)", "lang": "de"}], "type": "flow data set", "refObjectId": "a2b32f97-3fc7-4af2-b209-525bc6426f33", "version": "24.01.000", "uri": "../flows/a2b32f97-3fc7-4af2-b209-525bc6426f33.xml"}, "exchange direction": "OUTPUT", "other": {"anies": [{"value": "0", "module": "B6"}, {"name": "referenceToUnitGroupDataSet", "value": {"shortDescription": [{"value": "kg", "lang": "en"}], "type": "unit group data set", "refObjectId": "93a60a57-a4c8-11da-a746-0800200c9a66", "version": "03.00.000", "uri": "../unitgroups/93a60a57-a4c8-11da-a746-0800200c9a66.xml"}}]}, "resolvedFlowVersion": "38.00.000", "flowProperties": [], "typeOfFlow": "Other flow", "classification": {"classHierarchy": "Quantities / Environmental quantities / EPD EN 15804 / LCI indicators", "name": "GaBiCategories"}}, {"dataSetInternalID": 100167, "referenceToFlowDataSet": {"shortDescription": [{"value": "Materials for recycling  (MFR)", "lang": "en"}, {"value": "Stoffe zum Recycling (MFR)", "lang": "de"}], "type": "flow data set", "refObjectId": "d7fe48a5-4103-49c8-9aae-b0b5dfdbd6ae", "version": "24.01.000", "uri": "../flows/d7fe48a5-4103-49c8-9aae-b0b5dfdbd6ae.xml"}, "exchange direction": "OUTPUT", "other": {"anies": [{"value": "0", "module": "B6"}, {"name": "referenceToUnitGroupDataSet", "value": {"shortDescription": [{"value": "kg", "lang": "en"}], "type": "unit group data set", "refObjectId": "93a60a57-a4c8-11da-a746-0800200c9a66", "version": "03.00.000", "uri": "../unitgroups/93a60a57-a4c8-11da-a746-0800200c9a66.xml"}}]}, "resolvedFlowVersion": "38.00.000", "flowProperties": [], "typeOfFlow": "Other flow", "classification": {"classHierarchy": "Quantities / Environmental quantities / EPD EN 15804 / LCI indicators", "name": "GaBiCategories"}}, {"dataSetInternalID": 100168, "referenceToFlowDataSet": {"shortDescription": [{"value": "Materials for energy recovery (MER)", "lang": "en"}, {"value": "Stoffe für die Energierückgewinnung (MER)", "lang": "de"}], "type": "flow data set", "refObjectId": "59a9181c-3aaf-46ee-8b13-2b3723b6e447", "version": "24.01.000", "uri": "../flows/59a9181c-3aaf-46ee-8b13-2b3723b6e447.xml"}, "exchange direction": "OUTPUT", "other": {"anies": [{"value": "0", "module": "B6"}, {"name": "referenceToUnitGroupDataSet", "value": {"shortDescription": [{"value": "kg", "lang": "en"}], "type": "unit group data set", "refObjectId": "93a60a57-a4c8-11da-a746-0800200c9a66", "version": "03.00.000", "uri": "../unitgroups/93a60a57-a4c8-11da-a746-0800200c9a66.xml"}}]}, "resolvedFlowVersion": "38.00.000", "flowProperties": [], "typeOfFlow": "Other flow", "classification": {"classHierarchy": "Quantities / Environmental quantities / EPD EN 15804 / LCI indicators", "name": "GaBiCategories"}}, {"dataSetInternalID": 100169, "referenceToFlowDataSet": {"shortDescription": [{"value": "Exported electrical energy (EEE)", "lang": "en"}, {"value": "Exportierte elektrische Energie (EEE)", "lang": "de"}], "type": "flow data set", "refObjectId": "4da0c987-2b76-40d6-9e9e-82a017aaaf29", "version": "24.01.000", "uri": "../flows/4da0c987-2b76-40d6-9e9e-82a017aaaf29.xml"}, "exchange direction": "OUTPUT", "other": {"anies": [{"value": "0", "module": "B6"}, {"name": "referenceToUnitGroupDataSet", "value": {"shortDescription": [{"value": "MJ", "lang": "en"}], "type": "unit group data set", "refObjectId": "93a60a57-a3c8-11da-a746-0800200c9a66", "version": "03.00.000", "uri": "../unitgroups/93a60a57-a3c8-11da-a746-0800200c9a66.xml"}}]}, "resolvedFlowVersion": "38.00.000", "flowProperties": [], "typeOfFlow": "Other flow", "classification": {"classHierarchy": "Quantities / Environmental quantities / EPD EN 15804 / LCI indicators", "name": "GaBiCategories"}}, {"dataSetInternalID": 100170, "referenceToFlowDataSet": {"shortDescription": [{"value": "Exported thermal energy (EET)", "lang": "en"}, {"value": "Exportierte thermische Energie (EET)", "lang": "de"}], "type": "flow data set", "refObjectId": "98daf38a-7a79-46d3-9a37-2b7bd0955810", "version": "24.01.000", "uri": "../flows/98daf38a-7a79-46d3-9a37-2b7bd0955810.xml"}, "exchange direction": "OUTPUT", "other": {"anies": [{"value": "0", "module": "B6"}, {"name": "referenceToUnitGroupDataSet", "value": {"shortDescription": [{"value": "MJ", "lang": "en"}], "type": "unit group data set", "refObjectId": "93a60a57-a3c8-11da-a746-0800200c9a66", "version": "03.00.000", "uri": "../unitgroups/93a60a57-a3c8-11da-a746-0800200c9a66.xml"}}]}, "resolvedFlowVersion": "38.00.000", "flowProperties": [], "typeOfFlow": "Other flow", "classification": {"classHierarchy": "Quantities / Environmental quantities / EPD EN 15804 / LCI indicators", "name": "GaBiCategories"}}]}, "LCIAResults": {"LCIAResult": [{"referenceToLCIAMethodDataSet": {"shortDescription": [{"value": "Climate change", "lang": "en"}, {"value": "Globales Erwärmungspotenzial - total (GWP-total)", "lang": "de"}], "type": "LCIA method data set", "refObjectId": "a7ea142a-9749-11ed-a8fc-0242ac120002", "version": "24.01.000", "uri": "../lciamethods/a7ea142a-9749-11ed-a8fc-0242ac120002.xml"}, "other": {"anies": [{"value": "0.456329502859639", "module": "B6"}, {"name": "referenceToUnitGroupDataSet", "value": {"shortDescription": [{"value": "kg CO2 eq.", "lang": "en"}], "type": "unit group data set", "refObjectId": "1ebf3012-d0db-4de2-aefd-ef30cedb0be1", "version": "25.00.000", "uri": "../unitgroups/1ebf3012-d0db-4de2-aefd-ef30cedb0be1.xml"}}]}}, {"referenceToLCIAMethodDataSet": {"shortDescription": [{"value": "Climate change-Fossil", "lang": "en"}, {"value": "Globales Erwärmungspotenzial - fossil (GWP-fossil)", "lang": "de"}], "type": "LCIA method data set", "refObjectId": "a7ea19c0-9749-11ed-a8fc-0242ac120002", "version": "24.01.000", "uri": "../lciamethods/a7ea19c0-9749-11ed-a8fc-0242ac120002.xml"}, "other": {"anies": [{"value": "0.450780551345797", "module": "B6"}, {"name": "referenceToUnitGroupDataSet", "value": {"shortDescription": [{"value": "kg CO2 eq.", "lang": "en"}], "type": "unit group data set", "refObjectId": "1ebf3012-d0db-4de2-aefd-ef30cedb0be1", "version": "25.00.000", "uri": "../unitgroups/1ebf3012-d0db-4de2-aefd-ef30cedb0be1.xml"}}]}}, {"referenceToLCIAMethodDataSet": {"shortDescription": [{"value": "Climate change-Biogenic", "lang": "en"}, {"value": "Globales Erwärmungspotenzial - biogen (GWP-biogenic)", "lang": "de"}], "type": "LCIA method data set", "refObjectId": "a7ea186c-9749-11ed-a8fc-0242ac120002", "version": "24.01.000", "uri": "../lciamethods/a7ea186c-9749-11ed-a8fc-0242ac120002.xml"}, "other": {"anies": [{"value": "0.00546563500280182", "module": "B6"}, {"name": "referenceToUnitGroupDataSet", "value": {"shortDescription": [{"value": "kg CO2 eq.", "lang": "en"}], "type": "unit group data set", "refObjectId": "1ebf3012-d0db-4de2-aefd-ef30cedb0be1", "version": "25.00.000", "uri": "../unitgroups/1ebf3012-d0db-4de2-aefd-ef30cedb0be1.xml"}}]}}, {"referenceToLCIAMethodDataSet": {"shortDescription": [{"value": "Climate change-Land use and land use change", "lang": "en"}, {"value": "Globales Erwärmungspotenzial - luluc (GWP-luluc)", "lang": "de"}], "type": "LCIA method data set", "refObjectId": "a7ea1ae2-9749-11ed-a8fc-0242ac120002", "version": "24.01.000", "uri": "../lciamethods/a7ea1ae2-9749-11ed-a8fc-0242ac120002.xml"}, "other": {"anies": [{"value": "8.33165110403088E-5", "module": "B6"}, {"name": "referenceToUnitGroupDataSet", "value": {"shortDescription": [{"value": "kg CO2 eq.", "lang": "en"}], "type": "unit group data set", "refObjectId": "1ebf3012-d0db-4de2-aefd-ef30cedb0be1", "version": "25.00.000", "uri": "../unitgroups/1ebf3012-d0db-4de2-aefd-ef30cedb0be1.xml"}}]}}, {"referenceToLCIAMethodDataSet": {"shortDescription": [{"value": "Depletion potenzial of the stratospheric ozone layer (ODP)", "lang": "en"}, {"value": "Abbaupotenzial der stratosphärischen Ozonschicht (ODP)", "lang": "de"}], "type": "LCIA method data set", "refObjectId": "b5c629d6-def3-11e6-bf01-fe55135034f3", "version": "24.01.000", "uri": "../lciamethods/b5c629d6-def3-11e6-bf01-fe55135034f3.xml"}, "other": {"anies": [{"value": "1.18951498462156E-11", "module": "B6"}, {"name": "referenceToUnitGroupDataSet", "value": {"shortDescription": [{"value": "kg CFC-11 eq.", "lang": "en"}], "type": "unit group data set", "refObjectId": "d9e957c9-7309-4474-bf3a-7777df6c4e5b", "version": "25.00.000", "uri": "../unitgroups/d9e957c9-7309-4474-bf3a-7777df6c4e5b.xml"}}]}}, {"referenceToLCIAMethodDataSet": {"shortDescription": [{"value": "Acidifcation potential, Accumulated Exceedance (AP)", "lang": "en"}, {"value": "Versauerungspotenzial, kumulierte Überschreitung (AP)", "lang": "de"}], "type": "LCIA method data set", "refObjectId": "b5c611c6-def3-11e6-bf01-fe55135034f3", "version": "24.01.000", "uri": "../lciamethods/b5c611c6-def3-11e6-bf01-fe55135034f3.xml"}, "other": {"anies": [{"value": "0.000693898798903765", "module": "B6"}, {"name": "referenceToUnitGroupDataSet", "value": {"shortDescription": [{"value": "Mole of H+ eq.", "lang": "en"}], "type": "unit group data set", "refObjectId": "42e089ac-92bf-4bf2-8ca1-5fc40d18f2ed", "version": "00.01.000", "uri": "../unitgroups/42e089ac-92bf-4bf2-8ca1-5fc40d18f2ed.xml"}}]}}, {"referenceToLCIAMethodDataSet": {"shortDescription": [{"value": "Eutrophication, freshwater", "lang": "en"}, {"value": "Eutrophierungspotenzial - Süßwasser (EP-freshwater)", "lang": "de"}], "type": "LCIA method data set", "refObjectId": "b53ec18f-7377-4ad3-86eb-cc3f4f276b2b", "version": "24.01.000", "uri": "../lciamethods/b53ec18f-7377-4ad3-86eb-cc3f4f276b2b.xml"}, "other": {"anies": [{"value": "2.41929333060847E-6", "module": "B6"}, {"name": "referenceToUnitGroupDataSet", "value": {"shortDescription": [{"value": "kg P eq.", "lang": "en"}], "type": "unit group data set", "refObjectId": "0429039d-a61d-4590-ba67-aa4a20a810a1", "version": "25.00.000", "uri": "../unitgroups/0429039d-a61d-4590-ba67-aa4a20a810a1.xml"}}]}}, {"referenceToLCIAMethodDataSet": {"shortDescription": [{"value": "Eutrophication marine", "lang": "en"}, {"value": "Eutrophierungspotenzial - Salzwasser (EP-marine)", "lang": "de"}], "type": "LCIA method data set", "refObjectId": "b5c619fa-def3-11e6-bf01-fe55135034f3", "version": "24.01.000", "uri": "../lciamethods/b5c619fa-def3-11e6-bf01-fe55135034f3.xml"}, "other": {"anies": [{"value": "0.000210508160347166", "module": "B6"}, {"name": "referenceToUnitGroupDataSet", "value": {"shortDescription": [{"value": "kg N eq.", "lang": "en"}], "type": "unit group data set", "refObjectId": "d05bb823-ecdf-4686-8c40-bf1d9257859f", "version": "00.00.003", "uri": "../unitgroups/d05bb823-ecdf-4686-8c40-bf1d9257859f.xml"}}]}}, {"referenceToLCIAMethodDataSet": {"shortDescription": [{"value": "Eutrophication, terrestrial", "lang": "en"}, {"value": "Eutrophierungspotenzial - Land (EP-terrestrial)", "lang": "de"}], "type": "LCIA method data set", "refObjectId": "b5c614d2-def3-11e6-bf01-fe55135034f3", "version": "24.01.000", "uri": "../lciamethods/b5c614d2-def3-11e6-bf01-fe55135034f3.xml"}, "other": {"anies": [{"value": "0.00217810257750808", "module": "B6"}, {"name": "referenceToUnitGroupDataSet", "value": {"shortDescription": [{"value": "Mole of N eq.", "lang": "en"}], "type": "unit group data set", "refObjectId": "71b4d617-0ec9-4d3f-b65e-e438940c2401", "version": "00.00.003", "uri": "../unitgroups/71b4d617-0ec9-4d3f-b65e-e438940c2401.xml"}}]}}, {"referenceToLCIAMethodDataSet": {"shortDescription": [{"value": "Photochemical Ozone Creation Potential  (POCP)", "lang": "en"}, {"value": "Bildungspotenzial für troposphärisches Ozon (POCP)", "lang": "de"}], "type": "LCIA method data set", "refObjectId": "b5c610fe-def3-11e6-bf01-fe55135034f3", "version": "24.01.000", "uri": "../lciamethods/b5c610fe-def3-11e6-bf01-fe55135034f3.xml"}, "other": {"anies": [{"value": "0.00051262591424402", "module": "B6"}, {"name": "referenceToUnitGroupDataSet", "value": {"shortDescription": [{"value": "kg NMVOC eq.", "lang": "en"}], "type": "unit group data set", "refObjectId": "d27c25f8-fbc1-44c6-b47b-4adbae4199c6", "version": "00.00.003", "uri": "../unitgroups/d27c25f8-fbc1-44c6-b47b-4adbae4199c6.xml"}}]}}, {"referenceToLCIAMethodDataSet": {"shortDescription": [{"value": "Resource use, minerals and metals", "lang": "en"}, {"value": "Potenzial für die Verknappung abiotischer Ressourcen  nicht fossile Ressourcen (ADPE)", "lang": "de"}], "type": "LCIA method data set", "refObjectId": "b2ad6494-c78d-11e6-9d9d-cec0c932ce01", "version": "24.01.000", "uri": "../lciamethods/b2ad6494-c78d-11e6-9d9d-cec0c932ce01.xml"}, "other": {"anies": [{"value": "7.68174663559293E-8", "module": "B6"}, {"name": "referenceToUnitGroupDataSet", "value": {"shortDescription": [{"value": "kg Sb eq.", "lang": "en"}], "type": "unit group data set", "refObjectId": "54ccd2d9-a32a-4fc2-923d-f2c8c93e89d4", "version": "25.00.000", "uri": "../unitgroups/54ccd2d9-a32a-4fc2-923d-f2c8c93e89d4.xml"}}]}}, {"referenceToLCIAMethodDataSet": {"shortDescription": [{"value": "Resource use, fossils", "lang": "en"}, {"value": "Potenzial für die Verknappung abiotischer Ressourcen  fossile Brennstoffe (ADPF)", "lang": "de"}], "type": "LCIA method data set", "refObjectId": "b2ad6110-c78d-11e6-9d9d-cec0c932ce01", "version": "24.01.000", "uri": "../lciamethods/b2ad6110-c78d-11e6-9d9d-cec0c932ce01.xml"}, "other": {"anies": [{"value": "6.03080859143438", "module": "B6"}, {"name": "referenceToUnitGroupDataSet", "value": {"shortDescription": [{"value": "MJ", "lang": "en"}], "type": "unit group data set", "refObjectId": "93a60a57-a3c8-11da-a746-0800200c9a66", "version": "02.00.000", "uri": "../unitgroups/93a60a57-a3c8-11da-a746-0800200c9a66.xml"}}]}}, {"referenceToLCIAMethodDataSet": {"shortDescription": [{"value": "Water use", "lang": "en"}, {"value": "Wasser-Entzugspotenzial (Benutzer) (WDP)", "lang": "de"}], "type": "LCIA method data set", "refObjectId": "b2ad66ce-c78d-11e6-9d9d-cec0c932ce01", "version": "24.01.000", "uri": "../lciamethods/b2ad66ce-c78d-11e6-9d9d-cec0c932ce01.xml"}, "other": {"anies": [{"value": "0.012148163480533", "module": "B6"}, {"name": "referenceToUnitGroupDataSet", "value": {"shortDescription": [{"value": "m³ world equiv.", "lang": "en"}], "type": "unit group data set", "refObjectId": "6ae2df01-888e-46c8-b17d-49fa3869b476", "version": "00.00.003", "uri": "../unitgroups/6ae2df01-888e-46c8-b17d-49fa3869b476.xml"}}]}}]}, "otherAttributes": {"{http://www.indata.network/EPD/2019}epd-version": "1.2"}, "version": "1.1", "locations": "../ILCDLocations.xml"}