{"processInformation": {"dataSetInformation": {"UUID": "8cd435d4-54ad-48c0-8d9e-9015b491bb79", "name": {"baseName": [{"value": "Bachl ReXPS - Extruded Polystyrene (XPS) foam board", "lang": "en"}, {"value": "Bachl ReXPS - Extrudierte Polystyrol-Schaumstoffplatten", "lang": "de"}], "functionalUnitFlowProperties": [{"lang": "en"}]}, "classificationInformation": {"classification": [{"class": [{"value": "Dämmstoffe", "level": 0, "classId": "2"}, {"value": "Extrudiertes Polystyrol (XPS)", "level": 1, "classId": "2.3"}, {"value": "XPS weiß", "level": 2, "classId": "2.3.01"}], "name": "OEKOBAU.DAT"}, {"class": [{"value": "02 Building products", "level": 0}, {"value": "Thermal insulation products", "level": 1}, {"value": "Insulating materials made of foam plastics", "level": 2}], "name": "IBUCategories"}]}, "generalComment": [{"value": "Bachl ReXPS is an extruded polystyrene foam (XPS) made of 100% recycled and reclaimed polystyrene, manufactured according to EN 13164 and available in sheet form with a density range of 30-35 kg/m³. Bachl ReXPS panels are supplied with a butt edge or shiplap. The EPD only applies to an unlaminated product; Lamination and additional product treatment are not taken into account.Regulation (EU) No. 305/2011 (CPR) applies to placing the product on the market in the European Union/European Free Trade Association (EU/EFTA) (with the exception of Switzerland). The\nProduct requires a declaration of performance taking into account EN 13164:2012+A1:2015 Thermal insulation products for buildings - Factory made extruded polystyrene foam (XPS) products - Specification and CE marking. The respective national regulations apply to application and use.", "lang": "en"}], "other": {"anies": [{"scenario": [{"description": [{"value": "100% incineration", "lang": "en"}, {"value": "100% Verbrennung", "lang": "de"}], "name": "S1", "default": true}, {"description": [{"value": "100% recycling", "lang": "en"}, {"value": "100% Recycling", "lang": "de"}], "name": "S2"}, {"description": [{"value": "100% landfill", "lang": "en"}, {"value": "100% Deponie", "lang": "de"}], "name": "S3"}]}]}}, "quantitativeReference": {"referenceToReferenceFlow": [0]}, "time": {"referenceYear": 2022, "dataSetValidUntil": 2027, "other": {"anies": [{"name": "publicationDateOfEPD", "value": 1669766400000}]}}, "geography": {"locationOfOperationSupplyOrProduction": {"location": "DE"}}, "technology": {"technologyDescriptionAndIncludedProcesses": [{"value": "Bachl ReXPS is made of 100% recycled polystyrene produced by a continuous extrusion process. \nTechnical data: \nSound absorption coefficient and dynamic rigidity are not relevant for Bachl ReXPS because this insulation panel is not used to improve room acoustics or impact sound insulation.\n\nFor fire performance, these products except in \nScandinavia achieve the fire classification Euroclass E \naccording to EN 13501-1. \nDeclared unit: \nThe declared unit is 1 m3 of the Re-XPS insulation board. The density of the product is 32.7 kg/m³.", "lang": "en"}, {"value": "Bachl ReXPS besteht aus 100 % recyceltem Polystyrol, das in einem kontinuierlichen Extrusionsverfahren hergestellt wird. \n", "lang": "de"}], "technologicalApplicability": [{"value": "The variety of the performance properties of\nBachl ReXPS make it suitable for use in a large\nnumber of applications such as: perimeter insulation,\nfloor insulation including insulation of highly loaded\nindustrial floors, insulation of thermal bridges for\nexterior walls, insulation of cavity walls, agricultural\nbuilding ceiling insulation, prefabricated elements e.g.\nbuilding sandwich panels.", "lang": "en"}, {"value": "Die Vielfalt der Leistungseigenschaften von\nBachl ReXPS eignet sich für eine Vielzahl von\nAnwendungen wie: Perimeterdämmung,\nBodendämmung einschließlich der Dämmung von hochbelasteten\nIndustrieböden, Dämmung von Wärmebrücken für\nAußenwänden, Dämmung von Hohlwänden, Dämmung von\nDeckenisolierung, vorgefertigte Elemente wie z.B.\nSandwichelemente für Gebäude.", "lang": "de"}]}}, "modellingAndValidation": {"LCIMethodAndAllocation": {"typeOfDataSet": "EPD", "referenceToLCAMethodDetails": [{"shortDescription": [{"value": "Insulating materials made of foam plastics.pdf", "lang": "en"}], "type": "source data set", "refObjectId": "597ce6ba-3346-43f7-989f-99f23a997aa7"}], "other": {"anies": [{"name": "subType", "value": "specific dataset"}]}}, "dataSourcesTreatmentAndRepresentativeness": {"referenceToDataSource": [{"shortDescription": [{"value": "GaBi Database (all versions)", "lang": "en"}], "type": "source data set", "refObjectId": "28d74cc0-db8b-4d7e-bc44-5f6d56ce0c4a"}, {"shortDescription": [{"value": "GaBi Database Edition 2022, CUP 2022.01", "lang": "en"}], "type": "source data set", "refObjectId": "86f664e2-7dab-4722-aad7-4c5206a4123b"}], "useAdviceForDataSet": [{"value": "Scope: \nThe data have been provided by one production site based in Tittling, Germany for the year 2021. \nSystem boundary: \nType of EPD according to EN 15804: \"cradle to gate with options, modules C1–C4, and module D\". The following modules are declared: A1–A3, C, D and additional modules: A4 + A5.  \n\nProduction - Modules A1-A3\n\nThe product stage includes:\n\nRaw material supply (A1): polystyrene (PS) re-granulates recycled externally, polystyrene (PS) briquettes and their recycling process on-site, blowing agents, co-blowing agents, and flame retardants.\nTransport to the manufacturer (A2) \nManufacturing (A3), including provision of all\nmaterials, products and energy, as well as waste processing up to the end-of-waste state.\n\nConstruction stage - Modules A4-A5\n\nThe construction process stage includes:\n\nTransport to the construction site (A4) \n\nTreatment of packaging material (A5) credits for potential avoided burdens due to energy substitution of electricity and thermal energy generation are declared in module D. \n\nEnd-of-life stage– Modules C1-C4 and D\n\nThe end-of-life stage includes\nManual dismantling (C1)\nTransport to EoL (C2) \nWaste processing & disposal (C) with three 100 % scenarios (scenario 1: thermal treatment (C3/1); scenario 2: Recycling (C3/2); scenario 3: landfill (C4/3))\nReuse, recovery or recycling potential (D) - beyond system boundary. No credits were accounted from any of the EoL scenarios (C3/1, C3/2, or C4/3) in module D. The credits in D/1, D/2, and D/3 are solely accounting for the avoided burdens calculated by the inversion of electricity grid mix and thermal energy from natural gas during packaging treatment (A5).", "lang": "en"}], "other": {"anies": [{"name": "referenceToOriginalEPD", "value": {"shortDescription": {"value": "Bachl ReXPS - Extruded Polystyrene (XPS) foam board.pdf", "defaultValue": "Bachl ReXPS - Extruded Polystyrene (XPS) foam board.pdf", "lstrings": [{"lang": "en", "value": "Bachl ReXPS - Extruded Polystyrene (XPS) foam board.pdf"}]}, "type": "source data set", "uuid": {"uuid": "f70898d1-0d49-449d-b4e7-c46321dadf07"}, "refObjectId": "f70898d1-0d49-449d-b4e7-c46321dadf07", "resourceURLs": ["https://oekobaudat.de/OEKOBAU.DAT/resource/sources/f70898d1-0d49-449d-b4e7-c46321dadf07/Bachl_ReXPS_-_Extruded_Polystyrene_XPS_foam_board_15886.pdf?version=00.01.000"]}}]}}, "validation": {"review": [{"referenceToNameOfReviewerAndInstitution": [{"shortDescription": [{"value": "Institut Bauen und Umwelt e. V.", "lang": "en"}], "type": "contact data set", "refObjectId": "d111dbec-b024-4be5-86c5-752d6eb2cf95", "uri": "../contacts/d111dbec-b024-4be5-86c5-752d6eb2cf95.xml"}], "type": "Accredited third party review"}]}, "complianceDeclarations": {"compliance": [{"referenceToComplianceSystem": {"shortDescription": [{"value": "DIN EN 15804+A2", "lang": "en"}], "type": "source data set", "refObjectId": "c0016b33-8cf7-415c-ac6e-deba0d21440d", "uri": "../sources/c0016b33-8cf7-415c-ac6e-deba0d21440d.xml"}}, {"referenceToComplianceSystem": {"shortDescription": [{"value": "ISO 14025", "lang": "en"}], "type": "source data set", "refObjectId": "4f2eb655-6e44-4874-a95a-e28f5442cd4d", "uri": "../sources/4f2eb655-6e44-4874-a95a-e28f5442cd4d.xml"}}]}}, "administrativeInformation": {"commissionerAndGoal": {"referenceToCommissioner": [{"shortDescription": [{"value": "Karl Bachl Kunststoffverarbeitung GmbH & Co. KG", "lang": "en"}], "type": "contact data set", "refObjectId": "14474393-68b0-40e4-b480-5346378d4751", "uri": "../contacts/14474393-68b0-40e4-b480-5346378d4751.xml"}]}, "dataGenerator": {"referenceToPersonOrEntityGeneratingTheDataSet": [{"shortDescription": [{"value": "Sphera Solutions GmbH", "lang": "en"}], "type": "contact data set", "refObjectId": "623edf96-39d1-4e6f-9892-674c7228546b", "uri": "../contacts/623edf96-39d1-4e6f-9892-674c7228546b.xml"}]}, "dataEntryBy": {"timeStamp": 1669796711967, "referenceToDataSetFormat": [{"shortDescription": [{"value": "ILCD Format", "lang": "en"}], "type": "source data set", "refObjectId": "a97a0155-0234-4b87-b4ce-a45da52f2a40", "uri": "../sources/a97a0155-0234-4b87-b4ce-a45da52f2a40.xml"}, {"shortDescription": [{"value": "EPD-Datenformaterweiterungen v1.2", "lang": "de"}, {"value": "EPD Data Format Extensions v1.2", "lang": "en"}], "type": "source data set", "refObjectId": "a29449fd-aa2f-4de8-b5d7-4b06b43c6fde", "uri": "../sources/a29449fd-aa2f-4de8-b5d7-4b06b43c6fde.xml"}]}, "publicationAndOwnership": {"dataSetVersion": "00.01.000", "referenceToRegistrationAuthority": {"shortDescription": [{"value": "Institut Bauen und Umwelt e. V.", "lang": "en"}], "type": "contact data set", "refObjectId": "d111dbec-b024-4be5-86c5-752d6eb2cf95", "uri": "../contacts/d111dbec-b024-4be5-86c5-752d6eb2cf95.xml"}, "registrationNumber": "EPD-BAC-20220231-CBA1-EN", "referenceToOwnershipOfDataSet": {"shortDescription": [{"value": "Karl Bachl Kunststoffverarbeitung GmbH & Co. KG", "lang": "en"}], "type": "contact data set", "refObjectId": "14474393-68b0-40e4-b480-5346378d4751", "uri": "../contacts/14474393-68b0-40e4-b480-5346378d4751.xml"}, "copyright": true, "licenseType": "Free of charge for all users and uses", "accessRestrictions": [{"value": "None", "lang": "en"}], "other": {"anies": [{"name": "referenceToPublisher", "value": {"shortDescription": [{"value": "Institut Bauen und Umwelt e. V.", "lang": "en"}], "type": "contact data set", "refObjectId": "d111dbec-b024-4be5-86c5-752d6eb2cf95", "uri": "../contacts/d111dbec-b024-4be5-86c5-752d6eb2cf95.xml"}}]}}}, "exchanges": {"exchange": [{"dataSetInternalID": 0, "referenceToFlowDataSet": {"shortDescription": [{"value": "Bachl Re-XPS - Extruded polystyrene (XPS) foam board ()", "lang": "en"}], "type": "flow data set", "refObjectId": "e4969697-878b-c36a-cef3-5b3030b053c1", "uri": "../flows/e4969697-878b-c36a-cef3-5b3030b053c1.xml"}, "meanAmount": 1.0, "referencesToDataSource": {}, "referenceFlow": true, "resolvedFlowVersion": "00.01.000", "resultingflowAmount": 1.0, "flowProperties": [{"name": [{"lang": "en", "value": "Volume"}, {"lang": "de", "value": "Volumen"}], "uuid": "93a60a56-a3c8-22da-a746-0800200c9a66", "referenceFlowProperty": true, "meanValue": 1.0, "referenceUnit": "m3", "unitGroupUUID": "cd950537-0a98-4044-9ba7-9f9a68d0a504"}], "materialProperties": [{"name": "gross density", "value": "32.7", "unit": "kg/m^3", "unitDescription": "kilograms per cubic metre"}], "typeOfFlow": "Product flow", "classification": {"classHierarchy": "Dämmstoffe / Extrudiertes Polystyrol (XPS) / XPS weiß", "name": "OEKOBAU.DAT"}}, {"dataSetInternalID": 1, "referenceToFlowDataSet": {"shortDescription": [{"value": "Renewable primary energy as energy carrier (PERE)", "lang": "en"}, {"value": "Erneuerbare Primärenergie als Energieträger (PERE)", "lang": "de"}], "type": "flow data set", "refObjectId": "20f32be5-0398-4288-9b6d-accddd195317", "uri": "../flows/20f32be5-0398-4288-9b6d-accddd195317.xml"}, "exchange direction": "INPUT", "other": {"anies": [{"name": "referenceToUnitGroupDataSet", "value": {"shortDescription": [{"value": "MJ", "lang": "en"}], "type": "unit group data set", "refObjectId": "93a60a57-a3c8-11da-a746-0800200c9a66", "uri": "../unitgroups/93a60a57-a3c8-11da-a746-0800200c9a66.xml"}}, {"value": "69.3662340570049", "module": "A1-A3"}, {"value": "0.380564697823308", "module": "A4"}, {"value": "0.057320858356698", "module": "A5"}, {"value": "0", "module": "C1"}, {"value": "0.371853989685717", "module": "C2"}, {"value": "2.91095340873227", "module": "C3", "scenario": "S1"}, {"value": "47.1481094156143", "module": "C3", "scenario": "S2"}, {"value": "2.70343471790903", "module": "C4"}, {"value": "-4.62137284150507", "module": "D", "scenario": "S1"}, {"value": "-4.62137284150507", "module": "D", "scenario": "S2"}, {"value": "-4.62137284150507", "module": "D", "scenario": "S3"}]}, "resolvedFlowVersion": "38.00.000", "flowProperties": [], "typeOfFlow": "Other flow", "classification": {"classHierarchy": "Quantities", "name": "GaBiCategories"}}, {"dataSetInternalID": 2, "referenceToFlowDataSet": {"shortDescription": [{"value": "Renewable primary energy resources as material utilization (PERM)", "lang": "en"}, {"value": "Erneuerbare Primärenergie zur stofflichen Nutzung (PERM)", "lang": "de"}], "type": "flow data set", "refObjectId": "fb3ec0de-548d-4508-aea5-00b73bf6f702", "uri": "../flows/fb3ec0de-548d-4508-aea5-00b73bf6f702.xml"}, "exchange direction": "INPUT", "other": {"anies": [{"name": "referenceToUnitGroupDataSet", "value": {"shortDescription": [{"value": "MJ", "lang": "en"}], "type": "unit group data set", "refObjectId": "93a60a57-a3c8-11da-a746-0800200c9a66", "uri": "../unitgroups/93a60a57-a3c8-11da-a746-0800200c9a66.xml"}}, {"value": "0", "module": "A1-A3"}, {"value": "0", "module": "A4"}, {"value": "0", "module": "A5"}, {"value": "0", "module": "C1"}, {"value": "0", "module": "C2"}, {"value": "0", "module": "C3", "scenario": "S1"}, {"value": "0", "module": "C3", "scenario": "S2"}, {"value": "0", "module": "C4"}, {"value": "0", "module": "D", "scenario": "S1"}, {"value": "0", "module": "D", "scenario": "S2"}, {"value": "0", "module": "D", "scenario": "S3"}]}, "resolvedFlowVersion": "38.00.000", "flowProperties": [], "typeOfFlow": "Other flow", "classification": {"classHierarchy": "Quantities", "name": "GaBiCategories"}}, {"dataSetInternalID": 3, "referenceToFlowDataSet": {"shortDescription": [{"value": "Total use of renewable primary energy resources (PERT)", "lang": "en"}, {"value": "Total erneuerbare Primärenergie (PERT)", "lang": "de"}], "type": "flow data set", "refObjectId": "53f97275-fa8a-4cdd-9024-65936002acd0", "uri": "../flows/53f97275-fa8a-4cdd-9024-65936002acd0.xml"}, "exchange direction": "INPUT", "other": {"anies": [{"name": "referenceToUnitGroupDataSet", "value": {"shortDescription": [{"value": "MJ", "lang": "en"}], "type": "unit group data set", "refObjectId": "93a60a57-a3c8-11da-a746-0800200c9a66", "uri": "../unitgroups/93a60a57-a3c8-11da-a746-0800200c9a66.xml"}}, {"value": "69.3662340570049", "module": "A1-A3"}, {"value": "0.380564697823308", "module": "A4"}, {"value": "0.057320858356698", "module": "A5"}, {"value": "0", "module": "C1"}, {"value": "0.371853989685717", "module": "C2"}, {"value": "2.91095340873227", "module": "C3", "scenario": "S1"}, {"value": "47.1481094156143", "module": "C3", "scenario": "S2"}, {"value": "2.70343471790903", "module": "C4"}, {"value": "-4.62137284150507", "module": "D", "scenario": "S1"}, {"value": "-4.62137284150507", "module": "D", "scenario": "S2"}, {"value": "-4.62137284150507", "module": "D", "scenario": "S3"}]}, "resolvedFlowVersion": "38.00.000", "flowProperties": [], "typeOfFlow": "Other flow", "classification": {"classHierarchy": "Quantities / Environmental quantities / EPD EN 15804 / LCI indicators", "name": "GaBiCategories"}}, {"dataSetInternalID": 4, "referenceToFlowDataSet": {"shortDescription": [{"value": "Non renewable primary energy as energy carrier (PENRE)", "lang": "en"}, {"value": "Nicht-erneuerbare Primärenergie als Energieträger (PENRE)", "lang": "de"}], "type": "flow data set", "refObjectId": "ac857178-2b45-46ec-892a-a9a4332f0372", "uri": "../flows/ac857178-2b45-46ec-892a-a9a4332f0372.xml"}, "exchange direction": "INPUT", "other": {"anies": [{"name": "referenceToUnitGroupDataSet", "value": {"shortDescription": [{"value": "MJ", "lang": "en"}], "type": "unit group data set", "refObjectId": "93a60a57-a3c8-11da-a746-0800200c9a66", "uri": "../unitgroups/93a60a57-a3c8-11da-a746-0800200c9a66.xml"}}, {"value": "755.89911524491", "module": "A1-A3"}, {"value": "6.71034496308931", "module": "A4"}, {"value": "30.8791674468702", "module": "A5"}, {"value": "0", "module": "C1"}, {"value": "6.55675253370646", "module": "C2"}, {"value": "12.1569994986928", "module": "C3", "scenario": "S1"}, {"value": "84.9361415815311", "module": "C3", "scenario": "S2"}, {"value": "32.9003841652763", "module": "C4"}, {"value": "-16.7365525296792", "module": "D", "scenario": "S1"}, {"value": "-16.7365525296792", "module": "D", "scenario": "S2"}, {"value": "-16.7365525296792", "module": "D", "scenario": "S3"}]}, "resolvedFlowVersion": "38.00.000", "flowProperties": [], "typeOfFlow": "Other flow", "classification": {"classHierarchy": "Quantities", "name": "GaBiCategories"}}, {"dataSetInternalID": 5, "referenceToFlowDataSet": {"shortDescription": [{"value": "Non renewable primary energy as material utilization (PENRM)", "lang": "en"}, {"value": "Nicht-erneuerbare Primärenergie zur stofflichen Nutzung (PENRM)", "lang": "de"}], "type": "flow data set", "refObjectId": "1421caa0-679d-4bf4-b282-0eb850ccae27", "uri": "../flows/1421caa0-679d-4bf4-b282-0eb850ccae27.xml"}, "exchange direction": "INPUT", "other": {"anies": [{"name": "referenceToUnitGroupDataSet", "value": {"shortDescription": [{"value": "MJ", "lang": "en"}], "type": "unit group data set", "refObjectId": "93a60a57-a3c8-11da-a746-0800200c9a66", "uri": "../unitgroups/93a60a57-a3c8-11da-a746-0800200c9a66.xml"}}, {"value": "30.636", "module": "A1-A3"}, {"value": "0", "module": "A4"}, {"value": "-30.636", "module": "A5"}, {"value": "0", "module": "C1"}, {"value": "0", "module": "C2"}, {"value": "0", "module": "C3", "scenario": "S1"}, {"value": "0", "module": "C3", "scenario": "S2"}, {"value": "0", "module": "C4"}, {"value": "0", "module": "D", "scenario": "S1"}, {"value": "0", "module": "D", "scenario": "S2"}, {"value": "0", "module": "D", "scenario": "S3"}]}, "resolvedFlowVersion": "38.00.000", "flowProperties": [], "typeOfFlow": "Other flow", "classification": {"classHierarchy": "Quantities", "name": "GaBiCategories"}}, {"dataSetInternalID": 6, "referenceToFlowDataSet": {"shortDescription": [{"value": "Total use of non renewable primary energy resources (PENRT)", "lang": "en"}, {"value": "Total nicht erneuerbare Primärenergie (PENRT)", "lang": "de"}], "type": "flow data set", "refObjectId": "06159210-646b-4c8d-8583-da9b3b95a6c1", "uri": "../flows/06159210-646b-4c8d-8583-da9b3b95a6c1.xml"}, "exchange direction": "INPUT", "other": {"anies": [{"name": "referenceToUnitGroupDataSet", "value": {"shortDescription": [{"value": "MJ", "lang": "en"}], "type": "unit group data set", "refObjectId": "93a60a57-a3c8-11da-a746-0800200c9a66", "uri": "../unitgroups/93a60a57-a3c8-11da-a746-0800200c9a66.xml"}}, {"value": "786.535115244916", "module": "A1-A3"}, {"value": "6.71034496308931", "module": "A4"}, {"value": "0.243167446870181", "module": "A5"}, {"value": "0", "module": "C1"}, {"value": "6.55675253370646", "module": "C2"}, {"value": "12.1569994986928", "module": "C3", "scenario": "S1"}, {"value": "84.9361415815316", "module": "C3", "scenario": "S2"}, {"value": "32.9003841652766", "module": "C4"}, {"value": "-16.7365525296794", "module": "D", "scenario": "S1"}, {"value": "-16.7365525296793", "module": "D", "scenario": "S2"}, {"value": "-16.7365525296793", "module": "D", "scenario": "S3"}]}, "resolvedFlowVersion": "38.00.000", "flowProperties": [], "typeOfFlow": "Other flow", "classification": {"classHierarchy": "Quantities / Environmental quantities / EPD EN 15804 / LCI indicators", "name": "GaBiCategories"}}, {"dataSetInternalID": 7, "referenceToFlowDataSet": {"shortDescription": [{"value": "Use of secondary material (SM)", "lang": "en"}, {"value": "Einsatz von Sekundärstoffen (SM)", "lang": "de"}], "type": "flow data set", "refObjectId": "c6a1f35f-2d09-4f54-8dfb-97e502e1ce92", "uri": "../flows/c6a1f35f-2d09-4f54-8dfb-97e502e1ce92.xml"}, "exchange direction": "INPUT", "other": {"anies": [{"name": "referenceToUnitGroupDataSet", "value": {"shortDescription": [{"value": "kg", "lang": "en"}], "type": "unit group data set", "refObjectId": "ad38d542-3fe9-439d-9b95-2f5f7752acaf", "uri": "../unitgroups/ad38d542-3fe9-439d-9b95-2f5f7752acaf.xml"}}, {"value": "28.35", "module": "A1-A3"}, {"value": "0", "module": "A4"}, {"value": "0", "module": "A5"}, {"value": "0", "module": "C1"}, {"value": "0", "module": "C2"}, {"value": "0", "module": "C3", "scenario": "S1"}, {"value": "0", "module": "C3", "scenario": "S2"}, {"value": "0", "module": "C4"}, {"value": "0", "module": "D", "scenario": "S1"}, {"value": "0", "module": "D", "scenario": "S2"}, {"value": "0", "module": "D", "scenario": "S3"}]}, "resolvedFlowVersion": "38.00.000", "flowProperties": [], "typeOfFlow": "Other flow", "classification": {"classHierarchy": "Quantities / Environmental quantities / EPD EN 15804 / LCI indicators", "name": "GaBiCategories"}}, {"dataSetInternalID": 8, "referenceToFlowDataSet": {"shortDescription": [{"value": "Use of renewable secondary fuels (RSF)", "lang": "en"}, {"value": "Erneuerbare Sekundärbrennstoffe (RSF)", "lang": "de"}], "type": "flow data set", "refObjectId": "64333088-a55f-4aa2-9a31-c10b07816787", "uri": "../flows/64333088-a55f-4aa2-9a31-c10b07816787.xml"}, "exchange direction": "INPUT", "other": {"anies": [{"name": "referenceToUnitGroupDataSet", "value": {"shortDescription": [{"value": "MJ", "lang": "en"}], "type": "unit group data set", "refObjectId": "93a60a57-a3c8-11da-a746-0800200c9a66", "uri": "../unitgroups/93a60a57-a3c8-11da-a746-0800200c9a66.xml"}}, {"value": "0", "module": "A1-A3"}, {"value": "0", "module": "A4"}, {"value": "0", "module": "A5"}, {"value": "0", "module": "C1"}, {"value": "0", "module": "C2"}, {"value": "0", "module": "C3", "scenario": "S1"}, {"value": "0", "module": "C3", "scenario": "S2"}, {"value": "0", "module": "C4"}, {"value": "0", "module": "D", "scenario": "S1"}, {"value": "0", "module": "D", "scenario": "S2"}, {"value": "0", "module": "D", "scenario": "S3"}]}, "resolvedFlowVersion": "38.00.000", "flowProperties": [], "typeOfFlow": "Other flow", "classification": {"classHierarchy": "Quantities / Environmental quantities / EPD EN 15804 / LCI indicators", "name": "GaBiCategories"}}, {"dataSetInternalID": 9, "referenceToFlowDataSet": {"shortDescription": [{"value": "Use of non renewable secondary fuels (NRSF)", "lang": "en"}, {"value": "Nicht erneuerbare Sekundärbrennstoffe (NRSF)", "lang": "de"}], "type": "flow data set", "refObjectId": "89def144-d39a-4287-b86f-efde453ddcb2", "uri": "../flows/89def144-d39a-4287-b86f-efde453ddcb2.xml"}, "exchange direction": "INPUT", "other": {"anies": [{"name": "referenceToUnitGroupDataSet", "value": {"shortDescription": [{"value": "MJ", "lang": "en"}], "type": "unit group data set", "refObjectId": "93a60a57-a3c8-11da-a746-0800200c9a66", "uri": "../unitgroups/93a60a57-a3c8-11da-a746-0800200c9a66.xml"}}, {"value": "0", "module": "A1-A3"}, {"value": "0", "module": "A4"}, {"value": "0", "module": "A5"}, {"value": "0", "module": "C1"}, {"value": "0", "module": "C2"}, {"value": "0", "module": "C3", "scenario": "S1"}, {"value": "0", "module": "C3", "scenario": "S2"}, {"value": "0", "module": "C4"}, {"value": "0", "module": "D", "scenario": "S1"}, {"value": "0", "module": "D", "scenario": "S2"}, {"value": "0", "module": "D", "scenario": "S3"}]}, "resolvedFlowVersion": "38.00.000", "flowProperties": [], "typeOfFlow": "Other flow", "classification": {"classHierarchy": "Quantities / Environmental quantities / EPD EN 15804 / LCI indicators", "name": "GaBiCategories"}}, {"dataSetInternalID": 10, "referenceToFlowDataSet": {"shortDescription": [{"value": "Use of net fresh water (FW)", "lang": "en"}, {"value": "Einsatz von Süßwasserressourcen (FW)", "lang": "de"}], "type": "flow data set", "refObjectId": "3cf952c8-f3a4-461d-8c96-96456ca62246", "uri": "../flows/3cf952c8-f3a4-461d-8c96-96456ca62246.xml"}, "exchange direction": "INPUT", "other": {"anies": [{"name": "referenceToUnitGroupDataSet", "value": {"shortDescription": [{"value": "m^3", "lang": "en"}], "type": "unit group data set", "refObjectId": "cd950537-0a98-4044-9ba7-9f9a68d0a504", "uri": "../unitgroups/cd950537-0a98-4044-9ba7-9f9a68d0a504.xml"}}, {"value": "0.355480388419183", "module": "A1-A3"}, {"value": "0.000430399285559966", "module": "A4"}, {"value": "0.00450711180893672", "module": "A5"}, {"value": "0", "module": "C1"}, {"value": "0.000420547918419025", "module": "C2"}, {"value": "0.209528415286157", "module": "C3", "scenario": "S1"}, {"value": "0.0449764830923485", "module": "C3", "scenario": "S2"}, {"value": "0.000425681672110878", "module": "C4"}, {"value": "-0.0044422429815687", "module": "D", "scenario": "S1"}, {"value": "-0.00444224298156914", "module": "D", "scenario": "S2"}, {"value": "-0.00444224298156914", "module": "D", "scenario": "S3"}]}, "resolvedFlowVersion": "38.00.000", "flowProperties": [], "typeOfFlow": "Other flow", "classification": {"classHierarchy": "Quantities / Environmental quantities / EPD EN 15804 / LCI indicators", "name": "GaBiCategories"}}, {"dataSetInternalID": 11, "referenceToFlowDataSet": {"shortDescription": [{"value": "Hazardous waste disposed (HWD)", "lang": "en"}, {"value": "Gefährlicher Abfall zur Deponie (HWD)", "lang": "de"}], "type": "flow data set", "refObjectId": "430f9e0f-59b2-46a0-8e0d-55e0e84948fc", "uri": "../flows/430f9e0f-59b2-46a0-8e0d-55e0e84948fc.xml"}, "exchange direction": "OUTPUT", "other": {"anies": [{"name": "referenceToUnitGroupDataSet", "value": {"shortDescription": [{"value": "kg", "lang": "en"}], "type": "unit group data set", "refObjectId": "ad38d542-3fe9-439d-9b95-2f5f7752acaf", "uri": "../unitgroups/ad38d542-3fe9-439d-9b95-2f5f7752acaf.xml"}}, {"value": "5.98725392175687E-08", "module": "A1-A3"}, {"value": "3.21342290789893E-11", "module": "A4"}, {"value": "2.28784377311953E-11", "module": "A5"}, {"value": "0", "module": "C1"}, {"value": "3.13987118533123E-11", "module": "C2"}, {"value": "1.14081966128133E-09", "module": "C3", "scenario": "S1"}, {"value": "7.34972737829394E-09", "module": "C3", "scenario": "S2"}, {"value": "5.07256125031237E-09", "module": "C4"}, {"value": "-2.26146686990798E-09", "module": "D", "scenario": "S1"}, {"value": "-2.26146686990798E-09", "module": "D", "scenario": "S2"}, {"value": "-2.26146686990798E-09", "module": "D", "scenario": "S3"}]}, "resolvedFlowVersion": "38.00.000", "flowProperties": [], "typeOfFlow": "Other flow", "classification": {"classHierarchy": "Quantities / Environmental quantities / EPD EN 15804 / LCI indicators", "name": "GaBiCategories"}}, {"dataSetInternalID": 12, "referenceToFlowDataSet": {"shortDescription": [{"value": "Non hazardous waste disposed (NHWD)", "lang": "en"}, {"value": "Entsorgter nicht gefährlicher Abfall (NHWD)", "lang": "de"}], "type": "flow data set", "refObjectId": "b29ef66b-e286-4afa-949f-62f1a7b4d7fa", "uri": "../flows/b29ef66b-e286-4afa-949f-62f1a7b4d7fa.xml"}, "exchange direction": "OUTPUT", "other": {"anies": [{"name": "referenceToUnitGroupDataSet", "value": {"shortDescription": [{"value": "kg", "lang": "en"}], "type": "unit group data set", "refObjectId": "ad38d542-3fe9-439d-9b95-2f5f7752acaf", "uri": "../unitgroups/ad38d542-3fe9-439d-9b95-2f5f7752acaf.xml"}}, {"value": "1.30194017370916", "module": "A1-A3"}, {"value": "0.000961689268818195", "module": "A4"}, {"value": "0.0082679016492751", "module": "A5"}, {"value": "0", "module": "C1"}, {"value": "0.000939677257226886", "module": "C2"}, {"value": "0.62961627768512", "module": "C3", "scenario": "S1"}, {"value": "0.0639872711297903", "module": "C3", "scenario": "S2"}, {"value": "32.5698662927184", "module": "C4"}, {"value": "-0.00847795776796865", "module": "D", "scenario": "S1"}, {"value": "-0.00847795776796864", "module": "D", "scenario": "S2"}, {"value": "-0.00847795776796864", "module": "D", "scenario": "S3"}]}, "resolvedFlowVersion": "38.00.000", "flowProperties": [], "typeOfFlow": "Other flow", "classification": {"classHierarchy": "Quantities / Environmental quantities / EPD EN 15804 / LCI indicators", "name": "GaBiCategories"}}, {"dataSetInternalID": 13, "referenceToFlowDataSet": {"shortDescription": [{"value": "Radioactive waste disposed (RWD)", "lang": "en"}, {"value": "Entsorgter radioaktiver Abfall (RWD)", "lang": "de"}], "type": "flow data set", "refObjectId": "3449546e-52ad-4b39-b809-9fb77cea8ff6", "uri": "../flows/3449546e-52ad-4b39-b809-9fb77cea8ff6.xml"}, "exchange direction": "OUTPUT", "other": {"anies": [{"name": "referenceToUnitGroupDataSet", "value": {"shortDescription": [{"value": "kg", "lang": "en"}], "type": "unit group data set", "refObjectId": "ad38d542-3fe9-439d-9b95-2f5f7752acaf", "uri": "../unitgroups/ad38d542-3fe9-439d-9b95-2f5f7752acaf.xml"}}, {"value": "0.0413014827197804", "module": "A1-A3"}, {"value": "8.26496263653679E-06", "module": "A4"}, {"value": "1.47118835568625E-05", "module": "A5"}, {"value": "0", "module": "C1"}, {"value": "8.07578671531564E-06", "module": "C2"}, {"value": "0.000732742175905639", "module": "C3", "scenario": "S1"}, {"value": "0.0135763595250508", "module": "C3", "scenario": "S2"}, {"value": "0.000404064578844296", "module": "C4"}, {"value": "-0.00132525747422236", "module": "D", "scenario": "S1"}, {"value": "-0.00132525747422235", "module": "D", "scenario": "S2"}, {"value": "-0.00132525747422235", "module": "D", "scenario": "S3"}]}, "resolvedFlowVersion": "38.00.000", "flowProperties": [], "typeOfFlow": "Other flow", "classification": {"classHierarchy": "Quantities / Environmental quantities / EPD EN 15804 / LCI indicators", "name": "GaBiCategories"}}, {"dataSetInternalID": 14, "referenceToFlowDataSet": {"shortDescription": [{"value": "Components for re-use (CRU)", "lang": "en"}, {"value": "Komponenten für die Wiederverwendung (CRU)", "lang": "de"}], "type": "flow data set", "refObjectId": "a2b32f97-3fc7-4af2-b209-525bc6426f33", "uri": "../flows/a2b32f97-3fc7-4af2-b209-525bc6426f33.xml"}, "exchange direction": "OUTPUT", "other": {"anies": [{"name": "referenceToUnitGroupDataSet", "value": {"shortDescription": [{"value": "kg", "lang": "en"}], "type": "unit group data set", "refObjectId": "ad38d542-3fe9-439d-9b95-2f5f7752acaf", "uri": "../unitgroups/ad38d542-3fe9-439d-9b95-2f5f7752acaf.xml"}}, {"value": "0", "module": "A1-A3"}, {"value": "0", "module": "A4"}, {"value": "0", "module": "A5"}, {"value": "0", "module": "C1"}, {"value": "0", "module": "C2"}, {"value": "0", "module": "C3", "scenario": "S1"}, {"value": "0", "module": "C3", "scenario": "S2"}, {"value": "0", "module": "C4"}, {"value": "0", "module": "D", "scenario": "S1"}, {"value": "0", "module": "D", "scenario": "S2"}, {"value": "0", "module": "D", "scenario": "S3"}]}, "resolvedFlowVersion": "38.00.000", "flowProperties": [], "typeOfFlow": "Other flow", "classification": {"classHierarchy": "Quantities / Environmental quantities / EPD EN 15804 / LCI indicators", "name": "GaBiCategories"}}, {"dataSetInternalID": 15, "referenceToFlowDataSet": {"shortDescription": [{"value": "Materials for recycling (MFR)", "lang": "en"}, {"value": "Stoffe zum Recycling (MFR)", "lang": "de"}], "type": "flow data set", "refObjectId": "d7fe48a5-4103-49c8-9aae-b0b5dfdbd6ae", "uri": "../flows/d7fe48a5-4103-49c8-9aae-b0b5dfdbd6ae.xml"}, "exchange direction": "OUTPUT", "other": {"anies": [{"name": "referenceToUnitGroupDataSet", "value": {"shortDescription": [{"value": "kg", "lang": "en"}], "type": "unit group data set", "refObjectId": "ad38d542-3fe9-439d-9b95-2f5f7752acaf", "uri": "../unitgroups/ad38d542-3fe9-439d-9b95-2f5f7752acaf.xml"}}, {"value": "0", "module": "A1-A3"}, {"value": "0", "module": "A4"}, {"value": "0", "module": "A5"}, {"value": "0", "module": "C1"}, {"value": "0", "module": "C2"}, {"value": "0", "module": "C3", "scenario": "S1"}, {"value": "32.7", "module": "C3", "scenario": "S2"}, {"value": "0", "module": "C4"}, {"value": "0", "module": "D", "scenario": "S1"}, {"value": "0", "module": "D", "scenario": "S2"}, {"value": "0", "module": "D", "scenario": "S3"}]}, "resolvedFlowVersion": "38.00.000", "flowProperties": [], "typeOfFlow": "Other flow", "classification": {"classHierarchy": "Quantities / Environmental quantities / EPD EN 15804 / LCI indicators", "name": "GaBiCategories"}}, {"dataSetInternalID": 16, "referenceToFlowDataSet": {"shortDescription": [{"value": "Materials for energy recovery (MER)", "lang": "en"}, {"value": "Stoffe für die Energierückgewinnung (MER)", "lang": "de"}], "type": "flow data set", "refObjectId": "59a9181c-3aaf-46ee-8b13-2b3723b6e447", "uri": "../flows/59a9181c-3aaf-46ee-8b13-2b3723b6e447.xml"}, "exchange direction": "OUTPUT", "other": {"anies": [{"name": "referenceToUnitGroupDataSet", "value": {"shortDescription": [{"value": "kg", "lang": "en"}], "type": "unit group data set", "refObjectId": "ad38d542-3fe9-439d-9b95-2f5f7752acaf", "uri": "../unitgroups/ad38d542-3fe9-439d-9b95-2f5f7752acaf.xml"}}, {"value": "0", "module": "A1-A3"}, {"value": "0", "module": "A4"}, {"value": "0", "module": "A5"}, {"value": "0", "module": "C1"}, {"value": "0", "module": "C2"}, {"value": "0", "module": "C3", "scenario": "S1"}, {"value": "0", "module": "C3", "scenario": "S2"}, {"value": "0", "module": "C4"}, {"value": "0", "module": "D", "scenario": "S1"}, {"value": "0", "module": "D", "scenario": "S2"}, {"value": "0", "module": "D", "scenario": "S3"}]}, "resolvedFlowVersion": "38.00.000", "flowProperties": [], "typeOfFlow": "Other flow", "classification": {"classHierarchy": "Quantities / Environmental quantities / EPD EN 15804 / LCI indicators", "name": "GaBiCategories"}}, {"dataSetInternalID": 17, "referenceToFlowDataSet": {"shortDescription": [{"value": "Exported electrical energy (EEE)", "lang": "en"}, {"value": "Exportierte elektrische Energie (EEE)", "lang": "de"}], "type": "flow data set", "refObjectId": "4da0c987-2b76-40d6-9e9e-82a017aaaf29", "uri": "../flows/4da0c987-2b76-40d6-9e9e-82a017aaaf29.xml"}, "exchange direction": "OUTPUT", "other": {"anies": [{"name": "referenceToUnitGroupDataSet", "value": {"shortDescription": [{"value": "MJ", "lang": "en"}], "type": "unit group data set", "refObjectId": "93a60a57-a3c8-11da-a746-0800200c9a66", "uri": "../unitgroups/93a60a57-a3c8-11da-a746-0800200c9a66.xml"}}, {"value": "0", "module": "A1-A3"}, {"value": "0", "module": "A4"}, {"value": "4.44963923895632", "module": "A5"}, {"value": "0", "module": "C1"}, {"value": "0", "module": "C2"}, {"value": "198.268363906412", "module": "C3", "scenario": "S1"}, {"value": "0", "module": "C3", "scenario": "S2"}, {"value": "0", "module": "C4"}, {"value": "0", "module": "D", "scenario": "S1"}, {"value": "0", "module": "D", "scenario": "S2"}, {"value": "0", "module": "D", "scenario": "S3"}]}, "resolvedFlowVersion": "38.00.000", "flowProperties": [], "typeOfFlow": "Other flow", "classification": {"classHierarchy": "Quantities / Environmental quantities / EPD EN 15804 / LCI indicators", "name": "GaBiCategories"}}, {"dataSetInternalID": 18, "referenceToFlowDataSet": {"shortDescription": [{"value": "Exported thermal energy (EET)", "lang": "en"}, {"value": "Exportierte thermische Energie (EET)", "lang": "de"}], "type": "flow data set", "refObjectId": "98daf38a-7a79-46d3-9a37-2b7bd0955810", "uri": "../flows/98daf38a-7a79-46d3-9a37-2b7bd0955810.xml"}, "exchange direction": "OUTPUT", "other": {"anies": [{"name": "referenceToUnitGroupDataSet", "value": {"shortDescription": [{"value": "MJ", "lang": "en"}], "type": "unit group data set", "refObjectId": "93a60a57-a3c8-11da-a746-0800200c9a66", "uri": "../unitgroups/93a60a57-a3c8-11da-a746-0800200c9a66.xml"}}, {"value": "0", "module": "A1-A3"}, {"value": "0", "module": "A4"}, {"value": "7.91206989181843", "module": "A5"}, {"value": "0", "module": "C1"}, {"value": "0", "module": "C2"}, {"value": "353.380732856254", "module": "C3", "scenario": "S1"}, {"value": "0", "module": "C3", "scenario": "S2"}, {"value": "0", "module": "C4"}, {"value": "0", "module": "D", "scenario": "S1"}, {"value": "0", "module": "D", "scenario": "S2"}, {"value": "0", "module": "D", "scenario": "S3"}]}, "resolvedFlowVersion": "38.00.000", "flowProperties": [], "typeOfFlow": "Other flow", "classification": {"classHierarchy": "Quantities / Environmental quantities / EPD EN 15804 / LCI indicators", "name": "GaBiCategories"}}]}, "LCIAResults": {"LCIAResult": [{"referenceToLCIAMethodDataSet": {"shortDescription": [{"value": "Global Warming Potential total (GWP-total)", "lang": "en"}, {"value": "Globales Erwärmungspotenzial total (GWP-total)", "lang": "de"}], "type": "LCIA method data set", "refObjectId": "6a37f984-a4b3-458a-a20a-64418c145fa2", "uri": "../lciamethods/6a37f984-a4b3-458a-a20a-64418c145fa2.xml"}, "other": {"anies": [{"name": "referenceToUnitGroupDataSet", "value": {"shortDescription": [{"value": "kg CO_(2)-Äq.", "lang": "en"}], "type": "unit group data set", "refObjectId": "1ebf3012-d0db-4de2-aefd-ef30cedb0be1", "uri": "../unitgroups/1ebf3012-d0db-4de2-aefd-ef30cedb0be1.xml"}}, {"value": "54.2416173425411", "module": "A1-A3"}, {"value": "0.505978533743402", "module": "A4"}, {"value": "2.08579186454395", "module": "A5"}, {"value": "0", "module": "C1"}, {"value": "0.49439724058475", "module": "C2"}, {"value": "109.524872552716", "module": "C3", "scenario": "S1"}, {"value": "4.72339255275829", "module": "C3", "scenario": "S2"}, {"value": "2.29404350354312", "module": "C4"}, {"value": "-0.988747743213216", "module": "D", "scenario": "S1"}, {"value": "-0.988747743213215", "module": "D", "scenario": "S2"}, {"value": "-0.988747743213215", "module": "D", "scenario": "S3"}]}}, {"referenceToLCIAMethodDataSet": {"shortDescription": [{"value": "Global Warming Potential fossil fuels (GWP-fossil)", "lang": "en"}, {"value": "Globales Erwärmungspotenzial fossil (GWP-fossil)", "lang": "de"}], "type": "LCIA method data set", "refObjectId": "5f635281-343e-44fb-83df-1971b155e6b6", "uri": "../lciamethods/5f635281-343e-44fb-83df-1971b155e6b6.xml"}, "other": {"anies": [{"name": "referenceToUnitGroupDataSet", "value": {"shortDescription": [{"value": "kg CO_(2)-Äq.", "lang": "en"}], "type": "unit group data set", "refObjectId": "1ebf3012-d0db-4de2-aefd-ef30cedb0be1", "uri": "../unitgroups/1ebf3012-d0db-4de2-aefd-ef30cedb0be1.xml"}}, {"value": "53.5854457538056", "module": "A1-A3"}, {"value": "0.503032438067318", "module": "A4"}, {"value": "2.08572267256713", "module": "A5"}, {"value": "0", "module": "C1"}, {"value": "0.491518577804377", "module": "C2"}, {"value": "109.521475825962", "module": "C3", "scenario": "S1"}, {"value": "4.68025319491255", "module": "C3", "scenario": "S2"}, {"value": "2.31758120291474", "module": "C4"}, {"value": "-0.983588205848648", "module": "D", "scenario": "S1"}, {"value": "-0.983588205848647", "module": "D", "scenario": "S2"}, {"value": "-0.983588205848647", "module": "D", "scenario": "S3"}]}}, {"referenceToLCIAMethodDataSet": {"shortDescription": [{"value": "Global Warming Potential biogenic (GWP-biogenic)", "lang": "en"}, {"value": "Globales Erwärmungspotenzial biogen (GWP-biogenic)", "lang": "de"}], "type": "LCIA method data set", "refObjectId": "2356e1ab-0185-4db5-86e5-16de51c7485c", "uri": "../lciamethods/2356e1ab-0185-4db5-86e5-16de51c7485c.xml"}, "other": {"anies": [{"name": "referenceToUnitGroupDataSet", "value": {"shortDescription": [{"value": "kg CO_(2)-Äq.", "lang": "en"}], "type": "unit group data set", "refObjectId": "1ebf3012-d0db-4de2-aefd-ef30cedb0be1", "uri": "../unitgroups/1ebf3012-d0db-4de2-aefd-ef30cedb0be1.xml"}}, {"value": "0.629729117633922", "module": "A1-A3"}, {"value": "0.000153239917592734", "module": "A4"}, {"value": "6.69918372814759E-05", "module": "A5"}, {"value": "0", "module": "C1"}, {"value": "0.00014973242411051", "module": "C2"}, {"value": "0.00326822816088908", "module": "C3", "scenario": "S1"}, {"value": "0.042149522765073", "module": "C3", "scenario": "S2"}, {"value": "-0.0246659866726582", "module": "C4"}, {"value": "-0.0050509123910121", "module": "D", "scenario": "S1"}, {"value": "-0.00505091239101209", "module": "D", "scenario": "S2"}, {"value": "-0.00505091239101209", "module": "D", "scenario": "S3"}]}}, {"referenceToLCIAMethodDataSet": {"shortDescription": [{"value": "Global Warming Potential luluc (GWP-luluc)", "lang": "en"}, {"value": "Globales Erwärmungspotenzial luluc (GWP-luluc)", "lang": "de"}], "type": "LCIA method data set", "refObjectId": "4331bbdb-978a-490d-8707-eeb047f01a55", "uri": "../lciamethods/4331bbdb-978a-490d-8707-eeb047f01a55.xml"}, "other": {"anies": [{"name": "referenceToUnitGroupDataSet", "value": {"shortDescription": [{"value": "kg CO_(2)-Äq.", "lang": "en"}], "type": "unit group data set", "refObjectId": "1ebf3012-d0db-4de2-aefd-ef30cedb0be1", "uri": "../unitgroups/1ebf3012-d0db-4de2-aefd-ef30cedb0be1.xml"}}, {"value": "0.0264424711016876", "module": "A1-A3"}, {"value": "0.00279285575849096", "module": "A4"}, {"value": "2.20013954173603E-06", "module": "A5"}, {"value": "0", "module": "C1"}, {"value": "0.00272893035626171", "module": "C2"}, {"value": "0.000128498592863911", "module": "C3", "scenario": "S1"}, {"value": "0.000989835080670853", "module": "C3", "scenario": "S2"}, {"value": "0.00112828730103577", "module": "C4"}, {"value": "-0.000108624973556288", "module": "D", "scenario": "S1"}, {"value": "-0.000108624973556288", "module": "D", "scenario": "S2"}, {"value": "-0.000108624973556288", "module": "D", "scenario": "S3"}]}}, {"referenceToLCIAMethodDataSet": {"shortDescription": [{"value": "Depletion potential of the stratospheric ozone layer (ODP)", "lang": "en"}, {"value": "Abbau Potential der stratosphärischen Ozonschicht (ODP)", "lang": "de"}], "type": "LCIA method data set", "refObjectId": "b5c629d6-def3-11e6-bf01-fe55135034f3", "uri": "../lciamethods/b5c629d6-def3-11e6-bf01-fe55135034f3.xml"}, "other": {"anies": [{"name": "referenceToUnitGroupDataSet", "value": {"shortDescription": [{"value": "kg CFC11-Äq.", "lang": "en"}], "type": "unit group data set", "refObjectId": "d9e957c9-7309-4474-bf3a-7777df6c4e5b", "uri": "../unitgroups/d9e957c9-7309-4474-bf3a-7777df6c4e5b.xml"}}, {"value": "1.72094672599029E-10", "module": "A1-A3"}, {"value": "3.00122045315758E-14", "module": "A4"}, {"value": "8.93645019331017E-14", "module": "A5"}, {"value": "0", "module": "C1"}, {"value": "2.93252581181656E-14", "module": "C2"}, {"value": "4.58404766845644E-12", "module": "C3", "scenario": "S1"}, {"value": "6.85138485625513E-11", "module": "C3", "scenario": "S2"}, {"value": "3.11297071052921E-12", "module": "C4"}, {"value": "-6.68984792381944E-12", "module": "D", "scenario": "S1"}, {"value": "-6.68984792381943E-12", "module": "D", "scenario": "S2"}, {"value": "-6.68984792381943E-12", "module": "D", "scenario": "S3"}]}}, {"referenceToLCIAMethodDataSet": {"shortDescription": [{"value": "Acidification potential of land and water (AP)", "lang": "en"}, {"value": "Versauerungspotenzial von Boden und Wasser (AP)", "lang": "de"}], "type": "LCIA method data set", "refObjectId": "b5c611c6-def3-11e6-bf01-fe55135034f3", "uri": "../lciamethods/b5c611c6-def3-11e6-bf01-fe55135034f3.xml"}, "other": {"anies": [{"name": "referenceToUnitGroupDataSet", "value": {"shortDescription": [{"value": "mol H^(+)-Äq.", "lang": "en"}], "type": "unit group data set", "refObjectId": "42e089ac-92bf-4bf2-8ca1-5fc40d18f2ed", "uri": "../unitgroups/42e089ac-92bf-4bf2-8ca1-5fc40d18f2ed.xml"}}, {"value": "0.0927437886777657", "module": "A1-A3"}, {"value": "0.000476746532501729", "module": "A4"}, {"value": "0.000207085444891648", "module": "A5"}, {"value": "0", "module": "C1"}, {"value": "0.000465834327759712", "module": "C2"}, {"value": "0.0096355764842797", "module": "C3", "scenario": "S1"}, {"value": "0.0102732295469091", "module": "C3", "scenario": "S2"}, {"value": "0.0068687339713351", "module": "C4"}, {"value": "-0.00129824270638087", "module": "D", "scenario": "S1"}, {"value": "-0.00129824270638087", "module": "D", "scenario": "S2"}, {"value": "-0.00129824270638087", "module": "D", "scenario": "S3"}]}}, {"referenceToLCIAMethodDataSet": {"shortDescription": [{"value": "Eutrophication potential aquatic freshwater (EP-freshwater)", "lang": "en"}, {"value": "Eutrophierungspotenzial Süßwasser (EP-freshwater)", "lang": "de"}], "type": "LCIA method data set", "refObjectId": "b53ec18f-7377-4ad3-86eb-cc3f4f276b2b", "uri": "../lciamethods/b53ec18f-7377-4ad3-86eb-cc3f4f276b2b.xml"}, "other": {"anies": [{"name": "referenceToUnitGroupDataSet", "value": {"shortDescription": [{"value": "kg PO_(4)-Äq.", "lang": "en"}], "type": "unit group data set", "refObjectId": "0429039d-a61d-4590-ba67-aa4a20a810a1", "uri": "../unitgroups/0429039d-a61d-4590-ba67-aa4a20a810a1.xml"}}, {"value": "0.000104659984877688", "module": "A1-A3"}, {"value": "1.49527924902206E-06", "module": "A4"}, {"value": "2.08324109659875E-08", "module": "A5"}, {"value": "0", "module": "C1"}, {"value": "1.46105394857531E-06", "module": "C2"}, {"value": "1.07260207972614E-06", "module": "C3", "scenario": "S1"}, {"value": "1.36549221296706E-05", "module": "C3", "scenario": "S2"}, {"value": "0.000432625099038477", "module": "C4"}, {"value": "-1.36090593669381E-06", "module": "D", "scenario": "S1"}, {"value": "-1.36090593669381E-06", "module": "D", "scenario": "S2"}, {"value": "-1.36090593669381E-06", "module": "D", "scenario": "S3"}]}}, {"referenceToLCIAMethodDataSet": {"shortDescription": [{"value": "Eutrophication potential aquatic marine (EP-marine)", "lang": "en"}, {"value": "Eutrophierungspotenzial Salzwasser (EP-marine)", "lang": "de"}], "type": "LCIA method data set", "refObjectId": "b5c619fa-def3-11e6-bf01-fe55135034f3", "uri": "../lciamethods/b5c619fa-def3-11e6-bf01-fe55135034f3.xml"}, "other": {"anies": [{"name": "referenceToUnitGroupDataSet", "value": {"shortDescription": [{"value": "kg N-Äq.", "lang": "en"}], "type": "unit group data set", "refObjectId": "d05bb823-ecdf-4686-8c40-bf1d9257859f", "uri": "../unitgroups/d05bb823-ecdf-4686-8c40-bf1d9257859f.xml"}}, {"value": "0.0337445670364842", "module": "A1-A3"}, {"value": "0.000148533528048423", "module": "A4"}, {"value": "4.31844722110535E-05", "module": "A5"}, {"value": "0", "module": "C1"}, {"value": "0.000145133758656052", "module": "C2"}, {"value": "0.00211291821652235", "module": "C3", "scenario": "S1"}, {"value": "0.00230524216807324", "module": "C3", "scenario": "S2"}, {"value": "0.00151961721704246", "module": "C4"}, {"value": "-0.000351694161555714", "module": "D", "scenario": "S1"}, {"value": "-0.000351694161555713", "module": "D", "scenario": "S2"}, {"value": "-0.000351694161555713", "module": "D", "scenario": "S3"}]}}, {"referenceToLCIAMethodDataSet": {"shortDescription": [{"value": "Eutrophication potential terrestrial (EP-terrestrial)", "lang": "en"}, {"value": "Eutrophierungspotenzial Land (EP-terrestrial)", "lang": "de"}], "type": "LCIA method data set", "refObjectId": "b5c614d2-def3-11e6-bf01-fe55135034f3", "uri": "../lciamethods/b5c614d2-def3-11e6-bf01-fe55135034f3.xml"}, "other": {"anies": [{"name": "referenceToUnitGroupDataSet", "value": {"shortDescription": [{"value": "mol N-Äq.", "lang": "en"}], "type": "unit group data set", "refObjectId": "71b4d617-0ec9-4d3f-b65e-e438940c2401", "uri": "../unitgroups/71b4d617-0ec9-4d3f-b65e-e438940c2401.xml"}}, {"value": "0.376345213504446", "module": "A1-A3"}, {"value": "0.00178421151232737", "module": "A4"}, {"value": "0.000970123654225734", "module": "A5"}, {"value": "0", "module": "C1"}, {"value": "0.00174337286957225", "module": "C2"}, {"value": "0.0452107128041993", "module": "C3", "scenario": "S1"}, {"value": "0.0241845609219681", "module": "C3", "scenario": "S2"}, {"value": "0.0166665636151257", "module": "C4"}, {"value": "-0.00376610774166575", "module": "D", "scenario": "S1"}, {"value": "-0.00376610774166575", "module": "D", "scenario": "S2"}, {"value": "-0.00376610774166575", "module": "D", "scenario": "S3"}]}}, {"referenceToLCIAMethodDataSet": {"shortDescription": [{"value": "Formation potential of tropospheric ozone photochemical oxidants (POCP)", "lang": "en"}, {"value": "Bildungspotential für troposphärisches Ozon (POCP)", "lang": "de"}], "type": "LCIA method data set", "refObjectId": "b5c610fe-def3-11e6-bf01-fe55135034f3", "uri": "../lciamethods/b5c610fe-def3-11e6-bf01-fe55135034f3.xml"}, "other": {"anies": [{"name": "referenceToUnitGroupDataSet", "value": {"shortDescription": [{"value": "kg NMVOC-Äq.", "lang": "en"}], "type": "unit group data set", "refObjectId": "d27c25f8-fbc1-44c6-b47b-4adbae4199c6", "uri": "../unitgroups/d27c25f8-fbc1-44c6-b47b-4adbae4199c6.xml"}}, {"value": "0.444705202137617", "module": "A1-A3"}, {"value": "0.000415403129350068", "module": "A4"}, {"value": "0.000128583026345976", "module": "A5"}, {"value": "0", "module": "C1"}, {"value": "0.000405895007761526", "module": "C2"}, {"value": "0.00622607350354244", "module": "C3", "scenario": "S1"}, {"value": "0.00623100308024436", "module": "C3", "scenario": "S2"}, {"value": "0.00488857384328252", "module": "C4"}, {"value": "-0.000984054926215206", "module": "D", "scenario": "S1"}, {"value": "-0.000984054926215205", "module": "D", "scenario": "S2"}, {"value": "-0.000984054926215205", "module": "D", "scenario": "S3"}]}}, {"referenceToLCIAMethodDataSet": {"shortDescription": [{"value": "Abiotic depletion potential for non fossil resources (ADPE)", "lang": "en"}, {"value": "Potenzial für den abiotischen Abbau nicht fossiler Ressourcen (ADPE)", "lang": "de"}], "type": "LCIA method data set", "refObjectId": "b2ad6494-c78d-11e6-9d9d-cec0c932ce01", "uri": "../lciamethods/b2ad6494-c78d-11e6-9d9d-cec0c932ce01.xml"}, "other": {"anies": [{"name": "referenceToUnitGroupDataSet", "value": {"shortDescription": [{"value": "kg Sb-Äq.", "lang": "en"}], "type": "unit group data set", "refObjectId": "54ccd2d9-a32a-4fc2-923d-f2c8c93e89d4", "uri": "../unitgroups/54ccd2d9-a32a-4fc2-923d-f2c8c93e89d4.xml"}}, {"value": "4.93357339001592E-06", "module": "A1-A3"}, {"value": "4.18770523860859E-08", "module": "A4"}, {"value": "2.16357986370536E-09", "module": "A5"}, {"value": "0", "module": "C1"}, {"value": "4.09185326308793E-08", "module": "C2"}, {"value": "1.10893716712797E-07", "module": "C3", "scenario": "S1"}, {"value": "1.27530535035231E-06", "module": "C3", "scenario": "S2"}, {"value": "1.60721831847868E-07", "module": "C4"}, {"value": "-1.49022936339299E-07", "module": "D", "scenario": "S1"}, {"value": "-1.49022936339299E-07", "module": "D", "scenario": "S2"}, {"value": "-1.49022936339299E-07", "module": "D", "scenario": "S3"}]}}, {"referenceToLCIAMethodDataSet": {"shortDescription": [{"value": "Abiotic depletion potential for fossil resources (ADPF)", "lang": "en"}, {"value": "Potenzial für den abiotischen Abbau fossiler Brennstoffe (ADPF)", "lang": "de"}], "type": "LCIA method data set", "refObjectId": "b2ad6110-c78d-11e6-9d9d-cec0c932ce01", "uri": "../lciamethods/b2ad6110-c78d-11e6-9d9d-cec0c932ce01.xml"}, "other": {"anies": [{"name": "referenceToUnitGroupDataSet", "value": {"shortDescription": [{"value": "MJ", "lang": "en"}], "type": "unit group data set", "refObjectId": "93a60a57-a3c8-11da-a746-0800200c9a66", "uri": "../unitgroups/93a60a57-a3c8-11da-a746-0800200c9a66.xml"}}, {"value": "786.042540161719", "module": "A1-A3"}, {"value": "6.69433425134597", "module": "A4"}, {"value": "0.242971655754008", "module": "A5"}, {"value": "0", "module": "C1"}, {"value": "6.54110828957788", "module": "C2"}, {"value": "12.147261975817", "module": "C3", "scenario": "S1"}, {"value": "84.9144334009367", "module": "C3", "scenario": "S2"}, {"value": "32.8876766858904", "module": "C4"}, {"value": "-16.7342893435999", "module": "D", "scenario": "S1"}, {"value": "-16.7342893435999", "module": "D", "scenario": "S2"}, {"value": "-16.7342893435999", "module": "D", "scenario": "S3"}]}}, {"referenceToLCIAMethodDataSet": {"shortDescription": [{"value": "Water use (WDP)", "lang": "en"}, {"value": "Wassernutzung (WDP)", "lang": "de"}], "type": "LCIA method data set", "refObjectId": "b2ad66ce-c78d-11e6-9d9d-cec0c932ce01", "uri": "../lciamethods/b2ad66ce-c78d-11e6-9d9d-cec0c932ce01.xml"}, "other": {"anies": [{"name": "referenceToUnitGroupDataSet", "value": {"shortDescription": [{"value": "m^(3) world-Äq. deprived", "lang": "en"}], "type": "unit group data set", "refObjectId": "6ae2df01-888e-46c8-b17d-49fa3869b476", "uri": "../unitgroups/6ae2df01-888e-46c8-b17d-49fa3869b476.xml"}}, {"value": "1.89094522266641", "module": "A1-A3"}, {"value": "0.004493350780088", "module": "A4"}, {"value": "0.192425191757818", "module": "A5"}, {"value": "0", "module": "C1"}, {"value": "0.00439050291366977", "module": "C2"}, {"value": "8.9410198989095", "module": "C3", "scenario": "S1"}, {"value": "1.06747498754061", "module": "C3", "scenario": "S2"}, {"value": "-0.022848841151351", "module": "C4"}, {"value": "-0.105380123213092", "module": "D", "scenario": "S1"}, {"value": "-0.105380123213077", "module": "D", "scenario": "S2"}, {"value": "-0.105380123213077", "module": "D", "scenario": "S3"}]}}, {"referenceToLCIAMethodDataSet": {"shortDescription": [{"value": "Incidence of disease due to PM emissions (PM)", "lang": "en"}, {"value": "Auftreten von Krankheiten aufgrund von Feinstaubemissionen (PM)", "lang": "de"}], "type": "LCIA method data set", "refObjectId": "b5c602c6-def3-11e6-bf01-fe55135034f3", "uri": "../lciamethods/b5c602c6-def3-11e6-bf01-fe55135034f3.xml"}, "other": {"anies": [{"name": "referenceToUnitGroupDataSet", "value": {"shortDescription": [{"value": "Disease incidence", "lang": "en"}], "type": "unit group data set", "refObjectId": "3883559b-648f-4afc-8ba2-0bd24f3affa3", "uri": "../unitgroups/3883559b-648f-4afc-8ba2-0bd24f3affa3.xml"}}, {"value": "1.54849377676373E-06", "module": "A1-A3"}, {"value": "2.88386550570226E-09", "module": "A4"}, {"value": "1.20985987518605E-09", "module": "A5"}, {"value": "0", "module": "C1"}, {"value": "2.81785699027263E-09", "module": "C2"}, {"value": "5.60914938314854E-08", "module": "C3", "scenario": "S1"}, {"value": "8.51692999753763E-08", "module": "C3", "scenario": "S2"}, {"value": "6.6012098975617E-08", "module": "C4"}, {"value": "-1.07538199793373E-08", "module": "D", "scenario": "S1"}, {"value": "-1.07538199793373E-08", "module": "D", "scenario": "S2"}, {"value": "-1.07538199793373E-08", "module": "D", "scenario": "S3"}]}}, {"referenceToLCIAMethodDataSet": {"shortDescription": [{"value": "Human exposure efficiency relative to U235 (IR)", "lang": "en"}, {"value": "Wirkung durch Exposition des Menschen mit U235 (IR)", "lang": "de"}], "type": "LCIA method data set", "refObjectId": "b5c632be-def3-11e6-bf01-fe55135034f3", "uri": "../lciamethods/b5c632be-def3-11e6-bf01-fe55135034f3.xml"}, "other": {"anies": [{"name": "referenceToUnitGroupDataSet", "value": {"shortDescription": [{"value": "kBq U235-Äq.", "lang": "en"}], "type": "unit group data set", "refObjectId": "456b05bf-1415-44a9-9993-02452f554c09", "uri": "../unitgroups/456b05bf-1415-44a9-9993-02452f554c09.xml"}}, {"value": "3.44011676292795", "module": "A1-A3"}, {"value": "0.00121115560200501", "module": "A4"}, {"value": "0.00241460555521408", "module": "A5"}, {"value": "0", "module": "C1"}, {"value": "0.00118343357991883", "module": "C2"}, {"value": "0.119613270078725", "module": "C3", "scenario": "S1"}, {"value": "2.29993091971019", "module": "C3", "scenario": "S2"}, {"value": "0.0596467181399746", "module": "C4"}, {"value": "-0.224399121546436", "module": "D", "scenario": "S1"}, {"value": "-0.224399121546436", "module": "D", "scenario": "S2"}, {"value": "-0.224399121546436", "module": "D", "scenario": "S3"}]}}, {"referenceToLCIAMethodDataSet": {"shortDescription": [{"value": "Comparative toxic unit for ecosystems (ETP-fw)", "lang": "en"}, {"value": "Toxizitätsvergleichseinheit für Ökosysteme (ETP-fw)", "lang": "de"}], "type": "LCIA method data set", "refObjectId": "ee1082d1-b0f7-43ca-a1f0-21e2a4a74511", "uri": "../lciamethods/ee1082d1-b0f7-43ca-a1f0-21e2a4a74511.xml"}, "other": {"anies": [{"name": "referenceToUnitGroupDataSet", "value": {"shortDescription": [{"value": "CTUe", "lang": "en"}], "type": "unit group data set", "refObjectId": "aa959ded-f1eb-4efb-9c5c-2d60be36b3e6", "uri": "../unitgroups/aa959ded-f1eb-4efb-9c5c-2d60be36b3e6.xml"}}, {"value": "401.356514919374", "module": "A1-A3"}, {"value": "4.64752484867131", "module": "A4"}, {"value": "0.112479886858399", "module": "A5"}, {"value": "0", "module": "C1"}, {"value": "4.54114810708038", "module": "C2"}, {"value": "5.95908519148633", "module": "C3", "scenario": "S1"}, {"value": "37.1988739732473", "module": "C3", "scenario": "S2"}, {"value": "32.1836704982373", "module": "C4"}, {"value": "-3.693838175231", "module": "D", "scenario": "S1"}, {"value": "-3.69383817523099", "module": "D", "scenario": "S2"}, {"value": "-3.69383817523099", "module": "D", "scenario": "S3"}]}}, {"referenceToLCIAMethodDataSet": {"shortDescription": [{"value": "Comparative toxic unit for humans (carcinogenic) (HTP-c)", "lang": "en"}, {"value": "Toxizitätsvergleichseinheit für Menschen (krebserregend) (HTP-c)", "lang": "de"}], "type": "LCIA method data set", "refObjectId": "2299222a-bbd8-474f-9d4f-4dd1f18aea7c", "uri": "../lciamethods/2299222a-bbd8-474f-9d4f-4dd1f18aea7c.xml"}, "other": {"anies": [{"name": "referenceToUnitGroupDataSet", "value": {"shortDescription": [{"value": "CTUh", "lang": "en"}], "type": "unit group data set", "refObjectId": "d4c9523e-2d7e-49fd-8469-998f547d3a70", "uri": "../unitgroups/d4c9523e-2d7e-49fd-8469-998f547d3a70.xml"}}, {"value": "7.19652137284507E-09", "module": "A1-A3"}, {"value": "9.36716453654082E-11", "module": "A4"}, {"value": "1.3280038196257E-11", "module": "A5"}, {"value": "0", "module": "C1"}, {"value": "9.15276042385958E-11", "module": "C2"}, {"value": "6.00468105636009E-10", "module": "C3", "scenario": "S1"}, {"value": "1.06842557832315E-09", "module": "C3", "scenario": "S2"}, {"value": "1.44511680930355E-09", "module": "C4"}, {"value": "-1.69023742636932E-10", "module": "D", "scenario": "S1"}, {"value": "-1.69023742636932E-10", "module": "D", "scenario": "S2"}, {"value": "-1.69023742636932E-10", "module": "D", "scenario": "S3"}]}}, {"referenceToLCIAMethodDataSet": {"shortDescription": [{"value": "Comparative toxic unit for humans (noncarcinogenic) (HTP-nc)", "lang": "en"}, {"value": "Toxizitätsvergleichseinheit für Menschen (nicht krebserregend) (HTP-nc)", "lang": "de"}], "type": "LCIA method data set", "refObjectId": "3af763a5-b7a1-48c9-9cee-1f223481fcef", "uri": "../lciamethods/3af763a5-b7a1-48c9-9cee-1f223481fcef.xml"}, "other": {"anies": [{"name": "referenceToUnitGroupDataSet", "value": {"shortDescription": [{"value": "CTUh", "lang": "en"}], "type": "unit group data set", "refObjectId": "d4c9523e-2d7e-49fd-8469-998f547d3a70", "uri": "../unitgroups/d4c9523e-2d7e-49fd-8469-998f547d3a70.xml"}}, {"value": "3.97117277669555E-07", "module": "A1-A3"}, {"value": "4.84627595599324E-09", "module": "A4"}, {"value": "4.13542633638691E-10", "module": "A5"}, {"value": "0", "module": "C1"}, {"value": "4.73535001975076E-09", "module": "C2"}, {"value": "1.95164742495441E-08", "module": "C3", "scenario": "S1"}, {"value": "3.90773126676623E-08", "module": "C3", "scenario": "S2"}, {"value": "1.21118293582757E-07", "module": "C4"}, {"value": "-6.48939586968594E-09", "module": "D", "scenario": "S1"}, {"value": "-6.48939586968593E-09", "module": "D", "scenario": "S2"}, {"value": "-6.48939586968593E-09", "module": "D", "scenario": "S3"}]}}, {"referenceToLCIAMethodDataSet": {"shortDescription": [{"value": "Soil quality index (SQP)", "lang": "en"}, {"value": "Bodenqualitätsindex (SQP)", "lang": "de"}], "type": "LCIA method data set", "refObjectId": "b2ad6890-c78d-11e6-9d9d-cec0c932ce01", "uri": "../lciamethods/b2ad6890-c78d-11e6-9d9d-cec0c932ce01.xml"}, "other": {"anies": [{"name": "referenceToUnitGroupDataSet", "value": {"shortDescription": [{"value": "SQP", "lang": "en"}], "type": "unit group data set", "refObjectId": "f130951c-e67f-4f7f-8dd4-665de3974e18", "uri": "../unitgroups/f130951c-e67f-4f7f-8dd4-665de3974e18.xml"}}, {"value": "60.0734712503925", "module": "A1-A3"}, {"value": "2.30350957042895", "module": "A4"}, {"value": "0.0735267129484151", "module": "A5"}, {"value": "0", "module": "C1"}, {"value": "2.2507847652252", "module": "C2"}, {"value": "3.69087283810418", "module": "C3", "scenario": "S1"}, {"value": "30.6220488587394", "module": "C3", "scenario": "S2"}, {"value": "2.36626172624778", "module": "C4"}, {"value": "-3.00132421930618", "module": "D", "scenario": "S1"}, {"value": "-3.00132421930618", "module": "D", "scenario": "S2"}, {"value": "-3.00132421930618", "module": "D", "scenario": "S3"}]}}]}, "otherAttributes": {"{http://www.indata.network/EPD/2019}epd-version": "1.2"}, "version": "1.1", "locations": "../ILCDLocations.xml"}