{"processInformation": {"dataSetInformation": {"UUID": "8d51f336-2546-4fde-8f04-1e7738d47e41", "name": {"baseName": [{"value": "POLYREY HPL®", "lang": "en"}, {"value": "POLYREY HPL", "lang": "de"}], "functionalUnitFlowProperties": [{"lang": "en"}]}, "classificationInformation": {"classification": [{"class": [{"value": "Holz", "level": 0, "classId": "3"}, {"value": "Holzwerkstoffe", "level": 1, "classId": "3.2"}, {"value": "Wood-Plastic-Composites", "level": 2, "classId": "3.2.09"}], "name": "OEKOBAU.DAT"}, {"class": [{"value": "02 Building products", "level": 0}, {"value": "Interior facilitys", "level": 1}, {"value": "Decorative board for interior use", "level": 2}], "name": "IBUCategories"}]}, "generalComment": [{"value": "POLYREY HPL® panels are decorative high-pressure laminates (HPL) in accordance with EN 438 and ISO 4586. \n\nPOLYREY HPL® panels consist of layers of fibrous cellulose (usually paper) impregnated with thermosetting synthetic resins that cure under heat and high pressure.\nThe decorative layer is decorative paper impregnated with melamine resin and the core is composed of layers of kraft paper impregnated with phenolic resin.\nThe process, a simultaneous application of heat and high specific pressure enables the flow and subsequent curing of the thermosetting synthetic resins to obtain a homogeneous and non-porous material (bulk density ≥ 1.35 g/cm) with the required surface. \nEssentially, POLYREY HPL® consists of more than 60 % paper and the remaining approximately 30 to 40 % consists of phenol-formaldehyde resin for the core layers and melamine-formaldehyde resin for the decorative top layer.\n\nPOLYREY HPL® panels are characterised by their aesthetic qualities, strength, durability and functional performances. HPL sheets are available in a wide variety of colours, patterns and surface finishes. They are resistant to wear, impact, scratching, moisture, heat, staining and light resistance and possess good hygienic and anti-static properties. HPL are easy to clean and maintain.\n\nThin HPL are not self-supporting and require bonding to the substrate. Typically they are glued to wood-based substrates to form a HPL composite panel.\nPOLYREY HPL® boards are available in a variety of dimensions, thicknesses (0.6 to 2.0 mm) and surface finishes. If flame-retardant HPL is required, the brown laminate core can be provided with a halogen-free additive. \n\nPOLYREY surfaces have antibacterial properties thanks to a treatment based on an active biocidal substance: silver borophosphate glass. This contributes to surface hygiene. \n\nThe declared product is HPL thickness 0.8 mm and average grammage of 1.08 kg/m2 that represents the majority of HPL manufactured.", "lang": "en"}, {"value": "POLYREY HPL®-Platten sind dekorative Hochdrucklaminate (HPL) gemäß EN 438 und ISO 4586. \n\nPOLYREY HPL®-Platten bestehen aus Schichten faseriger Zellulose (in der Regel Papier), die mit wärmehärtenden Kunstharzen imprägniert sind, die unter Hitze und hohem Druck aushärten. Die Dekorschicht ist mit Melaminharz imprägniertes Dekorpapier und der Kern besteht aus Schichten von mit Phenolharz imprägniertem Kraftpapier. Das Verfahren, eine gleichzeitige Anwendung von Hitze und hohem spezifischen Druck, ermöglicht das Fließen und anschließende Aushärten der wärmehärtenden Kunstharze, um ein homogenes und porenfreies Material (Schüttdichte ≥ 1,35 g/cm³) mit der gewünschten Oberfläche zu erhalten. \nIm Wesentlichen besteht POLYREY HPL® zu mehr als 60 % aus Papier und die restlichen ca. 30 bis 40 % aus Phenol-Formaldehyd-Harz für die Kernschichten und Melamin-Formaldehyd-Harz für die dekorative Deckschicht. POLYREY HPL®-Platten zeichnen sich durch ihre ästhetischen Qualitäten, ihre Festigkeit, Haltbarkeit und ihre funktionellen Leistungen aus. HPL-Platten sind in einer großen Auswahl an Farben, Mustern und Oberflächenbehandlungen erhältlich. Sie sind verschleißfest, stoßfest, kratzfest, feuchtigkeits-, hitze-, flecken- und lichtbeständig und verfügen über gute hygienische und antistatische Eigenschaften. HPL sind leicht zu reinigen und zu pflegen. Dünne HPL sind nicht selbsttragend und müssen mit dem Untergrund verklebt werden. In der Regel werden sie auf Holzwerkstoffe geklebt, um eine HPL-Verbundplatte zu bilden. POLYREY HPL®-Platten sind in einer Vielzahl von Abmessungen, Stärken (0,6 bis 2,0 mm) und Oberflächenausführungen erhältlich. Wenn flammhemmendes HPL erforderlich ist, kann der braune Laminatkern mit einem halogenfreien Zusatz versehen werden. \n\nDie Oberflächen von POLYREY haben dank einer Behandlung auf der Basis eines bioziden Wirkstoffs antibakterielle Eigenschaften: Silberborophosphatglas. Dies trägt zur Oberflächenhygiene bei. \n\nBei dem deklarierten Produkt handelt es sich um HPL mit einer Dicke von 0,8 mm und einem durchschnittlichen Gewicht von 1,08 kg/m2, das den Großteil des hergestellten HPL ausmacht.", "lang": "de"}]}, "quantitativeReference": {"referenceToReferenceFlow": [0]}, "time": {"referenceYear": 2025, "dataSetValidUntil": 2030, "other": {"anies": [{"name": "publicationDateOfEPD", "value": 1742947200000}]}}, "geography": {"locationOfOperationSupplyOrProduction": {"location": "RER"}}, "technology": {"technologyDescriptionAndIncludedProcesses": [{"value": "The manufacturing process involves resin production, resin treating and drying, collation and assembly, pressing, sanding, and cutting to size: Resin: Two resins are used in the production of POLYREY HPL® : phenol-formaldehyde and melamine-formaldehyde resins for treating of the core papers and for treatment of the overlay and decorative papers.The phenolic and melamine resins are produced on Polyrey's site. Resin Treating and Drying: During the treating and drying step, papers are mechanically fed through a resin bath and then heated in an oven to cure the resin. Collation and Assembly: During collation (of the core sheets) and assembly (of the decorative and overlay sheets) sheets of treated and untreated paper are stacked both manually and mechanically. This step is in preparation of the pressing stage. Pressing: During pressing, the collated core and assembled decorative/overlay sheets are brought together to be pressed into the laminate product using stainless steel plates and high temperature and pressure. The output of the pressing process is the laminate product. Untreated kraft paper is used as a protective layer and a thermal barrier between the textured metal plates and the heated press platens. Sanding and triming : During the sanding process, sanding belts are used to remove the release resin on the outside face of the laminate. During this finishing step, panels are trimed lenght and width to their standard size.Then panels are shipped in their standard size to the fabricator. \nTechnical data: \nPOLYREY HPL® are tested and assessed in accordance with EN 438-2. The product requirements can be found in Part 3 of the EN 438 series of standards. Further information can be found in the product data sheet available on our website http://www.polyrey.com. \nDeclared unit: \nThe declared unit is 1 m2 of HPL product with 0.8 mm thickness with a density of at least 1350 kg/m.", "lang": "en"}, {"value": "Der Herstellungsprozess umfasst die Harzproduktion, die Harzbehandlung und -trocknung, das Zusammenstellen und die Montage, das Pressen, das Schleifen und den Zuschnitt:\n\nHarz: Für die Herstellung von POLYREY HPL® werden zwei Harze verwendet: Phenol-Formaldehyd- und Melamin-Formaldehyd-Harze für die Behandlung der Kernpapiere und für die Behandlung der Overlay- und Dekorpapiere. Die Phenol- und Melaminharze werden im Werk von Polyrey hergestellt.\n\nBehandlung und Trocknung des Harzes: Während des Behandlungs- und Trocknungsschritts werden die Papiere mechanisch durch ein Harzbad geführt und anschließend in einem Ofen erhitzt, um das Harz zu härten.\n\nZusammentragen und Zusammenfügen: Während des Zusammentragens (der Kernblätter) und des Zusammenfügens (der Dekor- und Overlayblätter) werden Blätter aus behandeltem und unbehandeltem Papier sowohl manuell als auch maschinell gestapelt. Dieser Schritt dient der Vorbereitung des Pressvorgangs.\nPressen: Beim Pressen werden die zusammengetragenen Kern- und zusammengesetzten Dekor-/Overlay-Bögen zusammengeführt, um mit Hilfe von Edelstahlplatten unter hoher Temperatur und hohem Druck zu dem Laminatprodukt gepresst zu werden. Das Ergebnis des Pressvorgangs ist das Laminatprodukt. Unbehandeltes Kraftpapier wird als Schutzschicht und thermische Barriere zwischen den strukturierten Metallplatten und den beheizten Pressplatten verwendet.\n\nSchleifen und Beschneiden : Während des Schleifvorgangs werden Schleifbänder verwendet, um das Trennharz auf der Außenseite des Laminats zu entfernen. Bei diesem Arbeitsschritt werden die Platten in Länge und Breite auf ihre Standardgröße zugeschnitten und dann in ihrer Standardgröße an den Verarbeiter versandt. \nTechnische Daten: \nPOLYREY HPL® werden gemäß EN 438-2 getestet und bewertet. Die Produktanforderungen finden Sie in Teil 3 der Normenreihe EN 438. Weitere Informationen finden Sie im Produktdatenblatt, das Sie auf unserer Website http://www.polyrey.com finden. \nDeklarierte Einheit: \nDie deklarierte Einheit ist 1 m2 HPL-Produkt mit 0,8 mm Dicke und einer Dichte von mindestens 1350 kg/m³.", "lang": "de"}], "technologicalApplicability": [{"value": "POLYREY HPL® in accordance to EN 438-3 is a surface material with excellent properties such as durability, cleanability and resistance to wear, combined with a wide range of technical and creative possibilities. POLYREY HPL® is easy to work with and maintain, making it suitable for a wide range of applications. Typical applications include wall and door coverings, furniture fittings and coverings, and worktops.", "lang": "en"}, {"value": "POLYREY HPL® nach EN 438-3 ist ein Oberflächenmaterial mit ausgezeichneten Eigenschaften wie Haltbarkeit, Reinigungsfähigkeit und Verschleißfestigkeit, kombiniert mit einer Vielzahl von technischen und gestalterischen Möglichkeiten. POLYREY HPL® ist leicht zu bearbeiten und zu pflegen und eignet sich daher für eine Vielzahl von Anwendungen. Typische Anwendungen sind Wand- und Türverkleidungen, Möbelbeschläge und -verkleidungen sowie Arbeitsplatten.", "lang": "de"}]}}, "modellingAndValidation": {"LCIMethodAndAllocation": {"typeOfDataSet": "EPD", "referenceToLCAMethodDetails": [{"shortDescription": [{"value": "Decorative board for interior use.pdf", "lang": "en"}], "type": "source data set", "refObjectId": "c33de4b6-202d-491a-a636-2647d3efc547"}], "other": {"anies": [{"name": "subType", "value": "specific dataset"}]}}, "dataSourcesTreatmentAndRepresentativeness": {"referenceToDataSource": [{"shortDescription": [{"value": "GaBi Database (all versions)", "lang": "en"}], "type": "source data set", "refObjectId": "28d74cc0-db8b-4d7e-bc44-5f6d56ce0c4a"}, {"shortDescription": [{"value": "GaBi Database Edition 2022, CUP 2022.01", "lang": "en"}], "type": "source data set", "refObjectId": "86f664e2-7dab-4722-aad7-4c5206a4123b"}], "useAdviceForDataSet": [{"value": "Scope: \nThe declaration relates to decorative high-pressure laminates in accordance with EN 438-3 with the product name POLYREY HPL®, which are manufactured at the POLYREY Baneuil production site in France. The declaration covers the entire range of colours/decors. \nSystem boundary: \nThe life cycle assessment of POLYREY HPL® includes a cradle-to-gate with options and the additionnal modules are A4 and A5. \nThe following phases of the life cycle are taken into account in the analysis: \n\n• Production of pre-products, extraction of energy carriers, raw material transportation, manufacture of product and packaging materials are declared in modules A1-A3.\nWithin the factory boundaries, the production of phenolic and melamine resin, the impregnation of the papers, the pressing process in the multi-opening presses, the formatting and the back sanding including the packaging are taken into account. The electrical energy used is supplied by the French power grid. Thermal energy is provided as an energy carrier by natural gas, wood chips and production residues.\nProduction losses are considered and treated mainly by incineration for energy recovery.\n\n• The scenario for the transport of the product to the construction site is declared in module A4.\n\n• The treatment of packaging materials at installation, installation auxiliaries, as well as installation losses are declared in module A5.\n\n• The impacts associated with use and maintenance are outside of the system boundary and are not included in the scope of this LCA (B1 and B2).\n\n• The end-of-life scenario is declared in the EPD. They include manual dismantling (C1), transportation to waste processing (C2), and end-of-life scenario 100 % thermal treatment with energy recovery (C3). Credits for electricity and thermal energy, which result from energy recovery in modules A5 and C3, are declared in module D.\n\n• The CO2 incorporation in the product (from the sequestration in the paper material) is considered. The C-balance is closed by considering the biotic CO2 emissions according to the incorporation on the input side.", "lang": "en"}, {"value": "Gültigkeitsbereich: \nDie Deklaration bezieht sich auf dekorative Hochdrucklaminate nach EN 438-3 mit dem Produktnamen POLYREY HPL®, die am Produktionsstandort POLYREY Baneuil in Frankreich hergestellt werden. Die Deklaration umfasst die gesamte Palette der Farben/Dekore. \nSystemgrenze: \nDie Ökobilanz von POLYREY HPL® umfasst ein Cradle-to-Gate mit Optionen und die zusätzlichen Module sind A4 und A5. \nDie folgenden Phasen des Lebenszyklus werden in der Analyse berücksichtigt: - Die Herstellung von Vorprodukten, die Gewinnung von Energieträgern, der Transport von Rohstoffen, die Herstellung von Produkt- und Verpackungsmaterialien werden in den Modulen A1-A3 angegeben. Innerhalb der Werksgrenzen werden die Herstellung von Phenol- und Melaminharz, die Imprägnierung der Papiere, der Pressvorgang in den Mehretagenpressen, die Formatierung und der Hinterschliff einschließlich der Verpackung berücksichtigt. Die verwendete elektrische Energie wird aus dem französischen Stromnetz bezogen. Thermische Energie wird als Energieträger durch Erdgas, Holzspäne und Produktionsrückstände bereitgestellt. Produktionsverluste werden berücksichtigt und hauptsächlich durch Verbrennung zur Energierückgewinnung behandelt. - Das Szenario für den Transport des Produkts zur Baustelle wird in Modul A4 angegeben. - Die Behandlung von Verpackungsmaterialien bei der Installation, Installationshilfsmittel sowie Installationsverluste werden in Modul A5 angegeben. - Die mit der Nutzung und Wartung verbundenen Auswirkungen liegen außerhalb der Systemgrenze und werden nicht in den Rahmen dieser Ökobilanz einbezogen (B1 und B2). - Das Szenario für das Lebensende wird in der EPD angegeben. Dazu gehören die manuelle Demontage (C1), der Transport zur Abfallverarbeitung (C2) und das End-of-Life-Szenario 100 % thermische Behandlung mit Energierückgewinnung (C3). Gutschriften für Strom und thermische Energie, die aus der Energierückgewinnung in den Modulen A5 und C3 resultieren, werden in Modul D angegeben. - Der CO2-Eintrag in das Produkt (aus der Sequestrierung im Papiermaterial) wird berücksichtigt. Die C-Bilanz wird geschlossen, indem die biotischen CO2-Emissionen entsprechend der Einbindung auf der Input-Seite berücksichtigt werden.", "lang": "de"}], "other": {"anies": [{"name": "referenceToOriginalEPD", "value": {"shortDescription": {"value": "POLYREY HPL®.pdf", "defaultValue": "POLYREY HPL®.pdf", "lstrings": [{"lang": "en", "value": "POLYREY HPL®.pdf"}]}, "type": "source data set", "uuid": {"uuid": "fede0aa7-fa61-4784-b6b1-3a5ed877393e"}, "refObjectId": "fede0aa7-fa61-4784-b6b1-3a5ed877393e", "resourceURLs": ["https://oekobaudat.de/OEKOBAU.DAT/resource/sources/fede0aa7-fa61-4784-b6b1-3a5ed877393e/POLYREY_HPL_22258.pdf?version=00.01.000"]}}]}}, "validation": {"review": [{"referenceToNameOfReviewerAndInstitution": [{"shortDescription": [{"value": "Institut Bauen und Umwelt e. V.", "lang": "en"}], "type": "contact data set", "refObjectId": "d111dbec-b024-4be5-86c5-752d6eb2cf95", "uri": "../contacts/d111dbec-b024-4be5-86c5-752d6eb2cf95.xml"}], "type": "Accredited third party review"}]}, "complianceDeclarations": {"compliance": [{"referenceToComplianceSystem": {"shortDescription": [{"value": "DIN EN 15804+A2", "lang": "en"}], "type": "source data set", "refObjectId": "c0016b33-8cf7-415c-ac6e-deba0d21440d", "uri": "../sources/c0016b33-8cf7-415c-ac6e-deba0d21440d.xml"}}, {"referenceToComplianceSystem": {"shortDescription": [{"value": "ISO 14025", "lang": "en"}], "type": "source data set", "refObjectId": "4f2eb655-6e44-4874-a95a-e28f5442cd4d", "uri": "../sources/4f2eb655-6e44-4874-a95a-e28f5442cd4d.xml"}}]}}, "administrativeInformation": {"commissionerAndGoal": {"referenceToCommissioner": [{"shortDescription": [{"value": "WILSONART UK", "lang": "en"}], "type": "contact data set", "refObjectId": "212b4800-ed29-4adc-b90f-d61efba0d4aa", "uri": "../contacts/212b4800-ed29-4adc-b90f-d61efba0d4aa.xml"}]}, "dataGenerator": {"referenceToPersonOrEntityGeneratingTheDataSet": [{"shortDescription": [{"value": "WILSONART UK", "lang": "en"}], "type": "contact data set", "refObjectId": "212b4800-ed29-4adc-b90f-d61efba0d4aa", "uri": "../contacts/212b4800-ed29-4adc-b90f-d61efba0d4aa.xml"}]}, "dataEntryBy": {"timeStamp": 1742947200000, "referenceToDataSetFormat": [{"shortDescription": [{"value": "ILCD Format", "lang": "en"}], "type": "source data set", "refObjectId": "a97a0155-0234-4b87-b4ce-a45da52f2a40", "uri": "../sources/a97a0155-0234-4b87-b4ce-a45da52f2a40.xml"}, {"shortDescription": [{"value": "EPD-Datenformaterweiterungen v1.2", "lang": "de"}, {"value": "EPD Data Format Extensions v1.2", "lang": "en"}], "type": "source data set", "refObjectId": "a29449fd-aa2f-4de8-b5d7-4b06b43c6fde", "uri": "../sources/a29449fd-aa2f-4de8-b5d7-4b06b43c6fde.xml"}]}, "publicationAndOwnership": {"dataSetVersion": "00.01.000", "referenceToRegistrationAuthority": {"shortDescription": [{"value": "Institut Bauen und Umwelt e. V.", "lang": "en"}], "type": "contact data set", "refObjectId": "d111dbec-b024-4be5-86c5-752d6eb2cf95", "uri": "../contacts/d111dbec-b024-4be5-86c5-752d6eb2cf95.xml"}, "registrationNumber": "EPD-WIL-20240581-IBA1-EN", "referenceToOwnershipOfDataSet": {"shortDescription": [{"value": "WILSONART UK", "lang": "en"}], "type": "contact data set", "refObjectId": "212b4800-ed29-4adc-b90f-d61efba0d4aa", "uri": "../contacts/212b4800-ed29-4adc-b90f-d61efba0d4aa.xml"}, "copyright": true, "licenseType": "Free of charge for all users and uses", "accessRestrictions": [{"value": "None", "lang": "en"}], "other": {"anies": [{"name": "referenceToPublisher", "value": {"shortDescription": [{"value": "Institut Bauen und Umwelt e. V.", "lang": "en"}], "type": "contact data set", "refObjectId": "d111dbec-b024-4be5-86c5-752d6eb2cf95", "uri": "../contacts/d111dbec-b024-4be5-86c5-752d6eb2cf95.xml"}}]}}}, "exchanges": {"exchange": [{"dataSetInternalID": 0, "referenceToFlowDataSet": {"shortDescription": [{"value": "POLYREY HPL (Na)", "lang": "en"}], "type": "flow data set", "refObjectId": "0d86898c-8bb2-a694-5d0d-536679ea989f", "uri": "../flows/0d86898c-8bb2-a694-5d0d-536679ea989f.xml"}, "meanAmount": 1.0, "referencesToDataSource": {}, "referenceFlow": true, "resolvedFlowVersion": "00.01.000", "resultingflowAmount": 1.0, "flowProperties": [{"name": [{"lang": "de", "value": "Fläche"}, {"lang": "en", "value": "Area"}], "uuid": "93a60a56-a3c8-19da-a746-0800200c9a66", "referenceFlowProperty": true, "meanValue": 1.0, "referenceUnit": "qm", "unitGroupUUID": "c20a03d7-bd90-4569-bc94-66cfd364dfc8"}], "materialProperties": [{"name": "gross density", "value": "1350.0", "unit": "kg/m^3", "unitDescription": "kilograms per cubic metre"}, {"name": "grammage", "value": "1.08", "unit": "kg/m^2", "unitDescription": "kilograms per square meter"}, {"name": "layer thickness", "value": "8.0E-4", "unit": "m", "unitDescription": "meters"}], "typeOfFlow": "Product flow", "classification": {"classHierarchy": "Holz / Holzwerkstoffe / Wood-Plastic-Composites", "name": "OEKOBAU.DAT"}}, {"dataSetInternalID": 1, "referenceToFlowDataSet": {"shortDescription": [{"value": "Renewable primary energy as energy carrier (PERE)", "lang": "en"}, {"value": "Erneuerbare Primärenergie als Energieträger (PERE)", "lang": "de"}], "type": "flow data set", "refObjectId": "20f32be5-0398-4288-9b6d-accddd195317", "uri": "../flows/20f32be5-0398-4288-9b6d-accddd195317.xml"}, "exchange direction": "INPUT", "other": {"anies": [{"name": "referenceToUnitGroupDataSet", "value": {"shortDescription": [{"value": "MJ", "lang": "en"}], "type": "unit group data set", "refObjectId": "93a60a57-a3c8-11da-a746-0800200c9a66", "uri": "../unitgroups/93a60a57-a3c8-11da-a746-0800200c9a66.xml"}}, {"value": "17.0405254677529", "module": "A1-A3"}, {"value": "0.0854346177585329", "module": "A4"}, {"value": "2.43770935122401", "module": "A5"}, {"value": "0", "module": "C1"}, {"value": "0.00380706000444797", "module": "C2"}, {"value": "10.4233911802462", "module": "C3"}, {"value": "0", "module": "C4"}, {"value": "-2.5930477379665", "module": "D"}]}, "resolvedFlowVersion": "38.00.000", "flowProperties": [], "typeOfFlow": "Other flow", "classification": {"classHierarchy": "Quantities", "name": "GaBiCategories"}}, {"dataSetInternalID": 2, "referenceToFlowDataSet": {"shortDescription": [{"value": "Renewable primary energy resources as material utilization (PERM)", "lang": "en"}, {"value": "Erneuerbare Primärenergie zur stofflichen Nutzung (PERM)", "lang": "de"}], "type": "flow data set", "refObjectId": "fb3ec0de-548d-4508-aea5-00b73bf6f702", "uri": "../flows/fb3ec0de-548d-4508-aea5-00b73bf6f702.xml"}, "exchange direction": "INPUT", "other": {"anies": [{"name": "referenceToUnitGroupDataSet", "value": {"shortDescription": [{"value": "MJ", "lang": "en"}], "type": "unit group data set", "refObjectId": "93a60a57-a3c8-11da-a746-0800200c9a66", "uri": "../unitgroups/93a60a57-a3c8-11da-a746-0800200c9a66.xml"}}, {"value": "12.14064", "module": "A1-A3"}, {"value": "0", "module": "A4"}, {"value": "-2.42064", "module": "A5"}, {"value": "0", "module": "C1"}, {"value": "0", "module": "C2"}, {"value": "-9.72", "module": "C3"}, {"value": "0", "module": "C4"}, {"value": "0", "module": "D"}]}, "resolvedFlowVersion": "38.00.000", "flowProperties": [], "typeOfFlow": "Other flow", "classification": {"classHierarchy": "Quantities", "name": "GaBiCategories"}}, {"dataSetInternalID": 3, "referenceToFlowDataSet": {"shortDescription": [{"value": "Total use of renewable primary energy resources (PERT)", "lang": "en"}, {"value": "Total erneuerbare Primärenergie (PERT)", "lang": "de"}], "type": "flow data set", "refObjectId": "53f97275-fa8a-4cdd-9024-65936002acd0", "uri": "../flows/53f97275-fa8a-4cdd-9024-65936002acd0.xml"}, "exchange direction": "INPUT", "other": {"anies": [{"name": "referenceToUnitGroupDataSet", "value": {"shortDescription": [{"value": "MJ", "lang": "en"}], "type": "unit group data set", "refObjectId": "93a60a57-a3c8-11da-a746-0800200c9a66", "uri": "../unitgroups/93a60a57-a3c8-11da-a746-0800200c9a66.xml"}}, {"value": "29.1811654677529", "module": "A1-A3"}, {"value": "0.0854346177585329", "module": "A4"}, {"value": "0.017069351224007", "module": "A5"}, {"value": "0", "module": "C1"}, {"value": "0.00380706000444797", "module": "C2"}, {"value": "0.703391180246159", "module": "C3"}, {"value": "0", "module": "C4"}, {"value": "-2.5930477379665", "module": "D"}]}, "resolvedFlowVersion": "38.00.000", "flowProperties": [], "typeOfFlow": "Other flow", "classification": {"classHierarchy": "Quantities / Environmental quantities / EPD EN 15804 / LCI indicators", "name": "GaBiCategories"}}, {"dataSetInternalID": 4, "referenceToFlowDataSet": {"shortDescription": [{"value": "Non renewable primary energy as energy carrier (PENRE)", "lang": "en"}, {"value": "Nicht-erneuerbare Primärenergie als Energieträger (PENRE)", "lang": "de"}], "type": "flow data set", "refObjectId": "ac857178-2b45-46ec-892a-a9a4332f0372", "uri": "../flows/ac857178-2b45-46ec-892a-a9a4332f0372.xml"}, "exchange direction": "INPUT", "other": {"anies": [{"name": "referenceToUnitGroupDataSet", "value": {"shortDescription": [{"value": "MJ", "lang": "en"}], "type": "unit group data set", "refObjectId": "93a60a57-a3c8-11da-a746-0800200c9a66", "uri": "../unitgroups/93a60a57-a3c8-11da-a746-0800200c9a66.xml"}}, {"value": "38.4074379229063", "module": "A1-A3"}, {"value": "1.23753643837236", "module": "A4"}, {"value": "1.01930820810934", "module": "A5"}, {"value": "0", "module": "C1"}, {"value": "0.0551459771481665", "module": "C2"}, {"value": "12.3983883166457", "module": "C3"}, {"value": "0", "module": "C4"}, {"value": "-4.67131073821282", "module": "D"}]}, "resolvedFlowVersion": "38.00.000", "flowProperties": [], "typeOfFlow": "Other flow", "classification": {"classHierarchy": "Quantities", "name": "GaBiCategories"}}, {"dataSetInternalID": 5, "referenceToFlowDataSet": {"shortDescription": [{"value": "Non renewable primary energy as material utilization (PENRM)", "lang": "en"}, {"value": "Nicht-erneuerbare Primärenergie zur stofflichen Nutzung (PENRM)", "lang": "de"}], "type": "flow data set", "refObjectId": "1421caa0-679d-4bf4-b282-0eb850ccae27", "uri": "../flows/1421caa0-679d-4bf4-b282-0eb850ccae27.xml"}, "exchange direction": "INPUT", "other": {"anies": [{"name": "referenceToUnitGroupDataSet", "value": {"shortDescription": [{"value": "MJ", "lang": "en"}], "type": "unit group data set", "refObjectId": "93a60a57-a3c8-11da-a746-0800200c9a66", "uri": "../unitgroups/93a60a57-a3c8-11da-a746-0800200c9a66.xml"}}, {"value": "10.6625", "module": "A1-A3"}, {"value": "0", "module": "A4"}, {"value": "-0.9425", "module": "A5"}, {"value": "0", "module": "C1"}, {"value": "0", "module": "C2"}, {"value": "-9.72", "module": "C3"}, {"value": "0", "module": "C4"}, {"value": "0", "module": "D"}]}, "resolvedFlowVersion": "38.00.000", "flowProperties": [], "typeOfFlow": "Other flow", "classification": {"classHierarchy": "Quantities", "name": "GaBiCategories"}}, {"dataSetInternalID": 6, "referenceToFlowDataSet": {"shortDescription": [{"value": "Total use of non renewable primary energy resources (PENRT)", "lang": "en"}, {"value": "Total nicht erneuerbare Primärenergie (PENRT)", "lang": "de"}], "type": "flow data set", "refObjectId": "06159210-646b-4c8d-8583-da9b3b95a6c1", "uri": "../flows/06159210-646b-4c8d-8583-da9b3b95a6c1.xml"}, "exchange direction": "INPUT", "other": {"anies": [{"name": "referenceToUnitGroupDataSet", "value": {"shortDescription": [{"value": "MJ", "lang": "en"}], "type": "unit group data set", "refObjectId": "93a60a57-a3c8-11da-a746-0800200c9a66", "uri": "../unitgroups/93a60a57-a3c8-11da-a746-0800200c9a66.xml"}}, {"value": "49.0699379229065", "module": "A1-A3"}, {"value": "1.23753643837236", "module": "A4"}, {"value": "0.0768082081093412", "module": "A5"}, {"value": "0", "module": "C1"}, {"value": "0.0551459771481666", "module": "C2"}, {"value": "2.67838831664575", "module": "C3"}, {"value": "0", "module": "C4"}, {"value": "-4.67131073821285", "module": "D"}]}, "resolvedFlowVersion": "38.00.000", "flowProperties": [], "typeOfFlow": "Other flow", "classification": {"classHierarchy": "Quantities / Environmental quantities / EPD EN 15804 / LCI indicators", "name": "GaBiCategories"}}, {"dataSetInternalID": 7, "referenceToFlowDataSet": {"shortDescription": [{"value": "Use of secondary material (SM)", "lang": "en"}, {"value": "Einsatz von Sekundärstoffen (SM)", "lang": "de"}], "type": "flow data set", "refObjectId": "c6a1f35f-2d09-4f54-8dfb-97e502e1ce92", "uri": "../flows/c6a1f35f-2d09-4f54-8dfb-97e502e1ce92.xml"}, "exchange direction": "INPUT", "other": {"anies": [{"name": "referenceToUnitGroupDataSet", "value": {"shortDescription": [{"value": "kg", "lang": "en"}], "type": "unit group data set", "refObjectId": "ad38d542-3fe9-439d-9b95-2f5f7752acaf", "uri": "../unitgroups/ad38d542-3fe9-439d-9b95-2f5f7752acaf.xml"}}, {"value": "0.256", "module": "A1-A3"}, {"value": "0", "module": "A4"}, {"value": "0", "module": "A5"}, {"value": "0", "module": "C1"}, {"value": "0", "module": "C2"}, {"value": "0", "module": "C3"}, {"value": "0", "module": "C4"}, {"value": "0", "module": "D"}]}, "resolvedFlowVersion": "38.00.000", "flowProperties": [], "typeOfFlow": "Other flow", "classification": {"classHierarchy": "Quantities / Environmental quantities / EPD EN 15804 / LCI indicators", "name": "GaBiCategories"}}, {"dataSetInternalID": 8, "referenceToFlowDataSet": {"shortDescription": [{"value": "Use of renewable secondary fuels (RSF)", "lang": "en"}, {"value": "Erneuerbare Sekundärbrennstoffe (RSF)", "lang": "de"}], "type": "flow data set", "refObjectId": "64333088-a55f-4aa2-9a31-c10b07816787", "uri": "../flows/64333088-a55f-4aa2-9a31-c10b07816787.xml"}, "exchange direction": "INPUT", "other": {"anies": [{"name": "referenceToUnitGroupDataSet", "value": {"shortDescription": [{"value": "MJ", "lang": "en"}], "type": "unit group data set", "refObjectId": "93a60a57-a3c8-11da-a746-0800200c9a66", "uri": "../unitgroups/93a60a57-a3c8-11da-a746-0800200c9a66.xml"}}, {"value": "0", "module": "A1-A3"}, {"value": "0", "module": "A4"}, {"value": "0", "module": "A5"}, {"value": "0", "module": "C1"}, {"value": "0", "module": "C2"}, {"value": "0", "module": "C3"}, {"value": "0", "module": "C4"}, {"value": "0", "module": "D"}]}, "resolvedFlowVersion": "38.00.000", "flowProperties": [], "typeOfFlow": "Other flow", "classification": {"classHierarchy": "Quantities / Environmental quantities / EPD EN 15804 / LCI indicators", "name": "GaBiCategories"}}, {"dataSetInternalID": 9, "referenceToFlowDataSet": {"shortDescription": [{"value": "Use of non renewable secondary fuels (NRSF)", "lang": "en"}, {"value": "Nicht erneuerbare Sekundärbrennstoffe (NRSF)", "lang": "de"}], "type": "flow data set", "refObjectId": "89def144-d39a-4287-b86f-efde453ddcb2", "uri": "../flows/89def144-d39a-4287-b86f-efde453ddcb2.xml"}, "exchange direction": "INPUT", "other": {"anies": [{"name": "referenceToUnitGroupDataSet", "value": {"shortDescription": [{"value": "MJ", "lang": "en"}], "type": "unit group data set", "refObjectId": "93a60a57-a3c8-11da-a746-0800200c9a66", "uri": "../unitgroups/93a60a57-a3c8-11da-a746-0800200c9a66.xml"}}, {"value": "0", "module": "A1-A3"}, {"value": "0", "module": "A4"}, {"value": "0", "module": "A5"}, {"value": "0", "module": "C1"}, {"value": "0", "module": "C2"}, {"value": "0", "module": "C3"}, {"value": "0", "module": "C4"}, {"value": "0", "module": "D"}]}, "resolvedFlowVersion": "38.00.000", "flowProperties": [], "typeOfFlow": "Other flow", "classification": {"classHierarchy": "Quantities / Environmental quantities / EPD EN 15804 / LCI indicators", "name": "GaBiCategories"}}, {"dataSetInternalID": 10, "referenceToFlowDataSet": {"shortDescription": [{"value": "Use of net fresh water (FW)", "lang": "en"}, {"value": "Einsatz von Süßwasserressourcen (FW)", "lang": "de"}], "type": "flow data set", "refObjectId": "3cf952c8-f3a4-461d-8c96-96456ca62246", "uri": "../flows/3cf952c8-f3a4-461d-8c96-96456ca62246.xml"}, "exchange direction": "INPUT", "other": {"anies": [{"name": "referenceToUnitGroupDataSet", "value": {"shortDescription": [{"value": "m^3", "lang": "en"}], "type": "unit group data set", "refObjectId": "cd950537-0a98-4044-9ba7-9f9a68d0a504", "uri": "../unitgroups/cd950537-0a98-4044-9ba7-9f9a68d0a504.xml"}}, {"value": "0.0149686271158323", "module": "A1-A3"}, {"value": "9.86922589240612E-05", "module": "A4"}, {"value": "0.00070765027371185", "module": "A5"}, {"value": "0", "module": "C1"}, {"value": "4.39783499424494E-06", "module": "C2"}, {"value": "0.00508585409335294", "module": "C3"}, {"value": "0", "module": "C4"}, {"value": "-0.00247361281692663", "module": "D"}]}, "resolvedFlowVersion": "38.00.000", "flowProperties": [], "typeOfFlow": "Other flow", "classification": {"classHierarchy": "Quantities / Environmental quantities / EPD EN 15804 / LCI indicators", "name": "GaBiCategories"}}, {"dataSetInternalID": 11, "referenceToFlowDataSet": {"shortDescription": [{"value": "Hazardous waste disposed (HWD)", "lang": "en"}, {"value": "Gefährlicher Abfall zur Deponie (HWD)", "lang": "de"}], "type": "flow data set", "refObjectId": "430f9e0f-59b2-46a0-8e0d-55e0e84948fc", "uri": "../flows/430f9e0f-59b2-46a0-8e0d-55e0e84948fc.xml"}, "exchange direction": "OUTPUT", "other": {"anies": [{"name": "referenceToUnitGroupDataSet", "value": {"shortDescription": [{"value": "kg", "lang": "en"}], "type": "unit group data set", "refObjectId": "ad38d542-3fe9-439d-9b95-2f5f7752acaf", "uri": "../unitgroups/ad38d542-3fe9-439d-9b95-2f5f7752acaf.xml"}}, {"value": "2.31103224614132E-06", "module": "A1-A3"}, {"value": "6.54805519221424E-12", "module": "A4"}, {"value": "6.48528470705113E-12", "module": "A5"}, {"value": "0", "module": "C1"}, {"value": "2.91788500765041E-13", "module": "C2"}, {"value": "2.13411790212769E-10", "module": "C3"}, {"value": "0", "module": "C4"}, {"value": "-4.04219685352727E-10", "module": "D"}]}, "resolvedFlowVersion": "38.00.000", "flowProperties": [], "typeOfFlow": "Other flow", "classification": {"classHierarchy": "Quantities / Environmental quantities / EPD EN 15804 / LCI indicators", "name": "GaBiCategories"}}, {"dataSetInternalID": 12, "referenceToFlowDataSet": {"shortDescription": [{"value": "Non hazardous waste disposed (NHWD)", "lang": "en"}, {"value": "Entsorgter nicht gefährlicher Abfall (NHWD)", "lang": "de"}], "type": "flow data set", "refObjectId": "b29ef66b-e286-4afa-949f-62f1a7b4d7fa", "uri": "../flows/b29ef66b-e286-4afa-949f-62f1a7b4d7fa.xml"}, "exchange direction": "OUTPUT", "other": {"anies": [{"name": "referenceToUnitGroupDataSet", "value": {"shortDescription": [{"value": "kg", "lang": "en"}], "type": "unit group data set", "refObjectId": "ad38d542-3fe9-439d-9b95-2f5f7752acaf", "uri": "../unitgroups/ad38d542-3fe9-439d-9b95-2f5f7752acaf.xml"}}, {"value": "0.0566772642587311", "module": "A1-A3"}, {"value": "0.000201625481838418", "module": "A4"}, {"value": "0.00642791209774426", "module": "A5"}, {"value": "0", "module": "C1"}, {"value": "8.98465198210506E-06", "module": "C2"}, {"value": "0.863292885488249", "module": "C3"}, {"value": "0", "module": "C4"}, {"value": "-0.00351916653113567", "module": "D"}]}, "resolvedFlowVersion": "38.00.000", "flowProperties": [], "typeOfFlow": "Other flow", "classification": {"classHierarchy": "Quantities / Environmental quantities / EPD EN 15804 / LCI indicators", "name": "GaBiCategories"}}, {"dataSetInternalID": 13, "referenceToFlowDataSet": {"shortDescription": [{"value": "Radioactive waste disposed (RWD)", "lang": "en"}, {"value": "Entsorgter radioaktiver Abfall (RWD)", "lang": "de"}], "type": "flow data set", "refObjectId": "3449546e-52ad-4b39-b809-9fb77cea8ff6", "uri": "../flows/3449546e-52ad-4b39-b809-9fb77cea8ff6.xml"}, "exchange direction": "OUTPUT", "other": {"anies": [{"name": "referenceToUnitGroupDataSet", "value": {"shortDescription": [{"value": "kg", "lang": "en"}], "type": "unit group data set", "refObjectId": "ad38d542-3fe9-439d-9b95-2f5f7752acaf", "uri": "../unitgroups/ad38d542-3fe9-439d-9b95-2f5f7752acaf.xml"}}, {"value": "0.00197005576836917", "module": "A1-A3"}, {"value": "2.29722432097088E-06", "module": "A4"}, {"value": "3.78095642008881E-06", "module": "A5"}, {"value": "0", "module": "C1"}, {"value": "1.02366828143735E-07", "module": "C2"}, {"value": "8.9991318172064E-05", "module": "C3"}, {"value": "0", "module": "C4"}, {"value": "-0.00074667147405478", "module": "D"}]}, "resolvedFlowVersion": "38.00.000", "flowProperties": [], "typeOfFlow": "Other flow", "classification": {"classHierarchy": "Quantities / Environmental quantities / EPD EN 15804 / LCI indicators", "name": "GaBiCategories"}}, {"dataSetInternalID": 14, "referenceToFlowDataSet": {"shortDescription": [{"value": "Components for re-use (CRU)", "lang": "en"}, {"value": "Komponenten für die Wiederverwendung (CRU)", "lang": "de"}], "type": "flow data set", "refObjectId": "a2b32f97-3fc7-4af2-b209-525bc6426f33", "uri": "../flows/a2b32f97-3fc7-4af2-b209-525bc6426f33.xml"}, "exchange direction": "OUTPUT", "other": {"anies": [{"name": "referenceToUnitGroupDataSet", "value": {"shortDescription": [{"value": "kg", "lang": "en"}], "type": "unit group data set", "refObjectId": "ad38d542-3fe9-439d-9b95-2f5f7752acaf", "uri": "../unitgroups/ad38d542-3fe9-439d-9b95-2f5f7752acaf.xml"}}, {"value": "0", "module": "A1-A3"}, {"value": "0", "module": "A4"}, {"value": "0", "module": "A5"}, {"value": "0", "module": "C1"}, {"value": "0", "module": "C2"}, {"value": "0", "module": "C3"}, {"value": "0", "module": "C4"}, {"value": "0", "module": "D"}]}, "resolvedFlowVersion": "38.00.000", "flowProperties": [], "typeOfFlow": "Other flow", "classification": {"classHierarchy": "Quantities / Environmental quantities / EPD EN 15804 / LCI indicators", "name": "GaBiCategories"}}, {"dataSetInternalID": 15, "referenceToFlowDataSet": {"shortDescription": [{"value": "Materials for recycling (MFR)", "lang": "en"}, {"value": "Stoffe zum Recycling (MFR)", "lang": "de"}], "type": "flow data set", "refObjectId": "d7fe48a5-4103-49c8-9aae-b0b5dfdbd6ae", "uri": "../flows/d7fe48a5-4103-49c8-9aae-b0b5dfdbd6ae.xml"}, "exchange direction": "OUTPUT", "other": {"anies": [{"name": "referenceToUnitGroupDataSet", "value": {"shortDescription": [{"value": "kg", "lang": "en"}], "type": "unit group data set", "refObjectId": "ad38d542-3fe9-439d-9b95-2f5f7752acaf", "uri": "../unitgroups/ad38d542-3fe9-439d-9b95-2f5f7752acaf.xml"}}, {"value": "0.015", "module": "A1-A3"}, {"value": "0", "module": "A4"}, {"value": "0", "module": "A5"}, {"value": "0", "module": "C1"}, {"value": "0", "module": "C2"}, {"value": "0", "module": "C3"}, {"value": "0", "module": "C4"}, {"value": "0", "module": "D"}]}, "resolvedFlowVersion": "38.00.000", "flowProperties": [], "typeOfFlow": "Other flow", "classification": {"classHierarchy": "Quantities / Environmental quantities / EPD EN 15804 / LCI indicators", "name": "GaBiCategories"}}, {"dataSetInternalID": 16, "referenceToFlowDataSet": {"shortDescription": [{"value": "Materials for energy recovery (MER)", "lang": "en"}, {"value": "Stoffe für die Energierückgewinnung (MER)", "lang": "de"}], "type": "flow data set", "refObjectId": "59a9181c-3aaf-46ee-8b13-2b3723b6e447", "uri": "../flows/59a9181c-3aaf-46ee-8b13-2b3723b6e447.xml"}, "exchange direction": "OUTPUT", "other": {"anies": [{"name": "referenceToUnitGroupDataSet", "value": {"shortDescription": [{"value": "kg", "lang": "en"}], "type": "unit group data set", "refObjectId": "ad38d542-3fe9-439d-9b95-2f5f7752acaf", "uri": "../unitgroups/ad38d542-3fe9-439d-9b95-2f5f7752acaf.xml"}}, {"value": "0", "module": "A1-A3"}, {"value": "0", "module": "A4"}, {"value": "0", "module": "A5"}, {"value": "0", "module": "C1"}, {"value": "0", "module": "C2"}, {"value": "0", "module": "C3"}, {"value": "0", "module": "C4"}, {"value": "0", "module": "D"}]}, "resolvedFlowVersion": "38.00.000", "flowProperties": [], "typeOfFlow": "Other flow", "classification": {"classHierarchy": "Quantities / Environmental quantities / EPD EN 15804 / LCI indicators", "name": "GaBiCategories"}}, {"dataSetInternalID": 17, "referenceToFlowDataSet": {"shortDescription": [{"value": "Exported electrical energy (EEE)", "lang": "en"}, {"value": "Exportierte elektrische Energie (EEE)", "lang": "de"}], "type": "flow data set", "refObjectId": "4da0c987-2b76-40d6-9e9e-82a017aaaf29", "uri": "../flows/4da0c987-2b76-40d6-9e9e-82a017aaaf29.xml"}, "exchange direction": "OUTPUT", "other": {"anies": [{"name": "referenceToUnitGroupDataSet", "value": {"shortDescription": [{"value": "MJ", "lang": "en"}], "type": "unit group data set", "refObjectId": "93a60a57-a3c8-11da-a746-0800200c9a66", "uri": "../unitgroups/93a60a57-a3c8-11da-a746-0800200c9a66.xml"}}, {"value": "0", "module": "A1-A3"}, {"value": "0", "module": "A4"}, {"value": "0.444667571901515", "module": "A5"}, {"value": "0", "module": "C1"}, {"value": "0", "module": "C2"}, {"value": "2.06810139087652", "module": "C3"}, {"value": "0", "module": "C4"}, {"value": "0", "module": "D"}]}, "resolvedFlowVersion": "38.00.000", "flowProperties": [], "typeOfFlow": "Other flow", "classification": {"classHierarchy": "Quantities / Environmental quantities / EPD EN 15804 / LCI indicators", "name": "GaBiCategories"}}, {"dataSetInternalID": 18, "referenceToFlowDataSet": {"shortDescription": [{"value": "Exported thermal energy (EET)", "lang": "en"}, {"value": "Exportierte thermische Energie (EET)", "lang": "de"}], "type": "flow data set", "refObjectId": "98daf38a-7a79-46d3-9a37-2b7bd0955810", "uri": "../flows/98daf38a-7a79-46d3-9a37-2b7bd0955810.xml"}, "exchange direction": "OUTPUT", "other": {"anies": [{"name": "referenceToUnitGroupDataSet", "value": {"shortDescription": [{"value": "MJ", "lang": "en"}], "type": "unit group data set", "refObjectId": "93a60a57-a3c8-11da-a746-0800200c9a66", "uri": "../unitgroups/93a60a57-a3c8-11da-a746-0800200c9a66.xml"}}, {"value": "0", "module": "A1-A3"}, {"value": "0", "module": "A4"}, {"value": "0.797992211608765", "module": "A5"}, {"value": "0", "module": "C1"}, {"value": "0", "module": "C2"}, {"value": "3.76381469583567", "module": "C3"}, {"value": "0", "module": "C4"}, {"value": "0", "module": "D"}]}, "resolvedFlowVersion": "38.00.000", "flowProperties": [], "typeOfFlow": "Other flow", "classification": {"classHierarchy": "Quantities / Environmental quantities / EPD EN 15804 / LCI indicators", "name": "GaBiCategories"}}]}, "LCIAResults": {"LCIAResult": [{"referenceToLCIAMethodDataSet": {"shortDescription": [{"value": "Global Warming Potential total (GWP-total)", "lang": "en"}, {"value": "Globales Erwärmungspotenzial total (GWP-total)", "lang": "de"}], "type": "LCIA method data set", "refObjectId": "6a37f984-a4b3-458a-a20a-64418c145fa2", "uri": "../lciamethods/6a37f984-a4b3-458a-a20a-64418c145fa2.xml"}, "other": {"anies": [{"name": "referenceToUnitGroupDataSet", "value": {"shortDescription": [{"value": "kg CO_(2) eq", "lang": "en"}], "type": "unit group data set", "refObjectId": "1ebf3012-d0db-4de2-aefd-ef30cedb0be1", "uri": "../unitgroups/1ebf3012-d0db-4de2-aefd-ef30cedb0be1.xml"}}, {"value": "1.3362511266605", "module": "A1-A3"}, {"value": "0.0933370762622213", "module": "A4"}, {"value": "0.295926090464977", "module": "A5"}, {"value": "0", "module": "C1"}, {"value": "0.00415920219804018", "module": "C2"}, {"value": "2.48687517343179", "module": "C3"}, {"value": "0", "module": "C4"}, {"value": "-0.519701619139821", "module": "D"}]}}, {"referenceToLCIAMethodDataSet": {"shortDescription": [{"value": "Global Warming Potential fossil fuels (GWP-fossil)", "lang": "en"}, {"value": "Globales Erwärmungspotenzial fossil (GWP-fossil)", "lang": "de"}], "type": "LCIA method data set", "refObjectId": "5f635281-343e-44fb-83df-1971b155e6b6", "uri": "../lciamethods/5f635281-343e-44fb-83df-1971b155e6b6.xml"}, "other": {"anies": [{"name": "referenceToUnitGroupDataSet", "value": {"shortDescription": [{"value": "kg CO_(2) eq", "lang": "en"}], "type": "unit group data set", "refObjectId": "1ebf3012-d0db-4de2-aefd-ef30cedb0be1", "uri": "../unitgroups/1ebf3012-d0db-4de2-aefd-ef30cedb0be1.xml"}}, {"value": "2.72458856774382", "module": "A1-A3"}, {"value": "0.0923174576648626", "module": "A4"}, {"value": "0.0561910028645095", "module": "A5"}, {"value": "0", "module": "C1"}, {"value": "0.0041137668782174", "module": "C2"}, {"value": "1.37901136582106", "module": "C3"}, {"value": "0", "module": "C4"}, {"value": "-0.517329044381984", "module": "D"}]}}, {"referenceToLCIAMethodDataSet": {"shortDescription": [{"value": "Global Warming Potential biogenic (GWP-biogenic)", "lang": "en"}, {"value": "Globales Erwärmungspotenzial biogen (GWP-biogenic)", "lang": "de"}], "type": "LCIA method data set", "refObjectId": "2356e1ab-0185-4db5-86e5-16de51c7485c", "uri": "../lciamethods/2356e1ab-0185-4db5-86e5-16de51c7485c.xml"}, "other": {"anies": [{"name": "referenceToUnitGroupDataSet", "value": {"shortDescription": [{"value": "kg CO_(2) eq", "lang": "en"}], "type": "unit group data set", "refObjectId": "1ebf3012-d0db-4de2-aefd-ef30cedb0be1", "uri": "../unitgroups/1ebf3012-d0db-4de2-aefd-ef30cedb0be1.xml"}}, {"value": "-1.39097616480902", "module": "A1-A3"}, {"value": "0.000386864409816682", "module": "A4"}, {"value": "0.239730238251768", "module": "A5"}, {"value": "0", "module": "C1"}, {"value": "1.72391012027482E-05", "module": "C2"}, {"value": "1.10775429153559", "module": "C3"}, {"value": "0", "module": "C4"}, {"value": "-0.00231813589170425", "module": "D"}]}}, {"referenceToLCIAMethodDataSet": {"shortDescription": [{"value": "Global Warming Potential luluc (GWP-luluc)", "lang": "en"}, {"value": "Globales Erwärmungspotenzial luluc (GWP-luluc)", "lang": "de"}], "type": "LCIA method data set", "refObjectId": "4331bbdb-978a-490d-8707-eeb047f01a55", "uri": "../lciamethods/4331bbdb-978a-490d-8707-eeb047f01a55.xml"}, "other": {"anies": [{"name": "referenceToUnitGroupDataSet", "value": {"shortDescription": [{"value": "kg CO_(2) eq", "lang": "en"}], "type": "unit group data set", "refObjectId": "1ebf3012-d0db-4de2-aefd-ef30cedb0be1", "uri": "../unitgroups/1ebf3012-d0db-4de2-aefd-ef30cedb0be1.xml"}}, {"value": "0.00263872372570184", "module": "A1-A3"}, {"value": "0.000632754187542076", "module": "A4"}, {"value": "4.84934869842831E-06", "module": "A5"}, {"value": "0", "module": "C1"}, {"value": "2.81962186200314E-05", "module": "C2"}, {"value": "0.00010951607514763", "module": "C3"}, {"value": "0", "module": "C4"}, {"value": "-5.4438866132847E-05", "module": "D"}]}}, {"referenceToLCIAMethodDataSet": {"shortDescription": [{"value": "Depletion potential of the stratospheric ozone layer (ODP)", "lang": "en"}, {"value": "Abbau Potential der stratosphärischen Ozonschicht (ODP)", "lang": "de"}], "type": "LCIA method data set", "refObjectId": "b5c629d6-def3-11e6-bf01-fe55135034f3", "uri": "../lciamethods/b5c629d6-def3-11e6-bf01-fe55135034f3.xml"}, "other": {"anies": [{"name": "referenceToUnitGroupDataSet", "value": {"shortDescription": [{"value": "kg CFC11 eq", "lang": "en"}], "type": "unit group data set", "refObjectId": "d9e957c9-7309-4474-bf3a-7777df6c4e5b", "uri": "../unitgroups/d9e957c9-7309-4474-bf3a-7777df6c4e5b.xml"}}, {"value": "1.1282080841949E-10", "module": "A1-A3"}, {"value": "9.22111064701629E-15", "module": "A4"}, {"value": "2.74968968009311E-14", "module": "A5"}, {"value": "0", "module": "C1"}, {"value": "4.10902775266866E-16", "module": "C2"}, {"value": "1.40201064055883E-12", "module": "C3"}, {"value": "0", "module": "C4"}, {"value": "-3.76811885431968E-12", "module": "D"}]}}, {"referenceToLCIAMethodDataSet": {"shortDescription": [{"value": "Acidification potential of land and water (AP)", "lang": "en"}, {"value": "Versauerungspotenzial von Boden und Wasser (AP)", "lang": "de"}], "type": "LCIA method data set", "refObjectId": "b5c611c6-def3-11e6-bf01-fe55135034f3", "uri": "../lciamethods/b5c611c6-def3-11e6-bf01-fe55135034f3.xml"}, "other": {"anies": [{"name": "referenceToUnitGroupDataSet", "value": {"shortDescription": [{"value": "mol H^(+) eq", "lang": "en"}], "type": "unit group data set", "refObjectId": "42e089ac-92bf-4bf2-8ca1-5fc40d18f2ed", "uri": "../unitgroups/42e089ac-92bf-4bf2-8ca1-5fc40d18f2ed.xml"}}, {"value": "0.00580868723077997", "module": "A1-A3"}, {"value": "0.000104888132764194", "module": "A4"}, {"value": "4.13366812990931E-05", "module": "A5"}, {"value": "0", "module": "C1"}, {"value": "4.67392990879166E-06", "module": "C2"}, {"value": "0.000568901989701306", "module": "C3"}, {"value": "0", "module": "C4"}, {"value": "-0.000657206664095868", "module": "D"}]}}, {"referenceToLCIAMethodDataSet": {"shortDescription": [{"value": "Eutrophication potential aquatic freshwater (EP-freshwater)", "lang": "en"}, {"value": "Eutrophierungspotenzial Süßwasser (EP-freshwater)", "lang": "de"}], "type": "LCIA method data set", "refObjectId": "b53ec18f-7377-4ad3-86eb-cc3f4f276b2b", "uri": "../lciamethods/b53ec18f-7377-4ad3-86eb-cc3f4f276b2b.xml"}, "other": {"anies": [{"name": "referenceToUnitGroupDataSet", "value": {"shortDescription": [{"value": "kg P eq", "lang": "en"}], "type": "unit group data set", "refObjectId": "0429039d-a61d-4590-ba67-aa4a20a810a1", "uri": "../unitgroups/0429039d-a61d-4590-ba67-aa4a20a810a1.xml"}}, {"value": "2.31768954338156E-05", "module": "A1-A3"}, {"value": "3.35439741061016E-07", "module": "A4"}, {"value": "8.67978005016783E-09", "module": "A5"}, {"value": "0", "module": "C1"}, {"value": "1.49475617214689E-08", "module": "C2"}, {"value": "3.62172232241957E-07", "module": "C3"}, {"value": "0", "module": "C4"}, {"value": "-7.50992253545693E-07", "module": "D"}]}}, {"referenceToLCIAMethodDataSet": {"shortDescription": [{"value": "Eutrophication potential aquatic marine (EP-marine)", "lang": "en"}, {"value": "Eutrophierungspotenzial Salzwasser (EP-marine)", "lang": "de"}], "type": "LCIA method data set", "refObjectId": "b5c619fa-def3-11e6-bf01-fe55135034f3", "uri": "../lciamethods/b5c619fa-def3-11e6-bf01-fe55135034f3.xml"}, "other": {"anies": [{"name": "referenceToUnitGroupDataSet", "value": {"shortDescription": [{"value": "kg N eq", "lang": "en"}], "type": "unit group data set", "refObjectId": "d05bb823-ecdf-4686-8c40-bf1d9257859f", "uri": "../unitgroups/d05bb823-ecdf-4686-8c40-bf1d9257859f.xml"}}, {"value": "0.00283742881831603", "module": "A1-A3"}, {"value": "3.376557110243E-05", "module": "A4"}, {"value": "1.31401052544654E-05", "module": "A5"}, {"value": "0", "module": "C1"}, {"value": "1.50463077665689E-06", "module": "C2"}, {"value": "0.000194431063307981", "module": "C3"}, {"value": "0", "module": "C4"}, {"value": "-0.000171721949799907", "module": "D"}]}}, {"referenceToLCIAMethodDataSet": {"shortDescription": [{"value": "Eutrophication potential terrestrial (EP-terrestrial)", "lang": "en"}, {"value": "Eutrophierungspotenzial Land (EP-terrestrial)", "lang": "de"}], "type": "LCIA method data set", "refObjectId": "b5c614d2-def3-11e6-bf01-fe55135034f3", "uri": "../lciamethods/b5c614d2-def3-11e6-bf01-fe55135034f3.xml"}, "other": {"anies": [{"name": "referenceToUnitGroupDataSet", "value": {"shortDescription": [{"value": "mol N eq", "lang": "en"}], "type": "unit group data set", "refObjectId": "71b4d617-0ec9-4d3f-b65e-e438940c2401", "uri": "../unitgroups/71b4d617-0ec9-4d3f-b65e-e438940c2401.xml"}}, {"value": "0.0211942505878653", "module": "A1-A3"}, {"value": "0.000404396396726609", "module": "A4"}, {"value": "0.000194833675456958", "module": "A5"}, {"value": "0", "module": "C1"}, {"value": "1.80203457136318E-05", "module": "C2"}, {"value": "0.00242291030348095", "module": "C3"}, {"value": "0", "module": "C4"}, {"value": "-0.0018349502771871", "module": "D"}]}}, {"referenceToLCIAMethodDataSet": {"shortDescription": [{"value": "Formation potential of tropospheric ozone photochemical oxidants (POCP)", "lang": "en"}, {"value": "Bildungspotential für troposphärisches Ozon (POCP)", "lang": "de"}], "type": "LCIA method data set", "refObjectId": "b5c610fe-def3-11e6-bf01-fe55135034f3", "uri": "../lciamethods/b5c610fe-def3-11e6-bf01-fe55135034f3.xml"}, "other": {"anies": [{"name": "referenceToUnitGroupDataSet", "value": {"shortDescription": [{"value": "kg NMVOC eq", "lang": "en"}], "type": "unit group data set", "refObjectId": "d27c25f8-fbc1-44c6-b47b-4adbae4199c6", "uri": "../unitgroups/d27c25f8-fbc1-44c6-b47b-4adbae4199c6.xml"}}, {"value": "0.00604709029802957", "module": "A1-A3"}, {"value": "9.03167744335554E-05", "module": "A4"}, {"value": "3.59580441689805E-05", "module": "A5"}, {"value": "0", "module": "C1"}, {"value": "4.02461424534665E-06", "module": "C2"}, {"value": "0.000542496088144195", "module": "C3"}, {"value": "0", "module": "C4"}, {"value": "-0.000466705723338162", "module": "D"}]}}, {"referenceToLCIAMethodDataSet": {"shortDescription": [{"value": "Abiotic depletion potential for non fossil resources (ADPE)", "lang": "en"}, {"value": "Potenzial für den abiotischen Abbau nicht fossiler Ressourcen (ADPE)", "lang": "de"}], "type": "LCIA method data set", "refObjectId": "b2ad6494-c78d-11e6-9d9d-cec0c932ce01", "uri": "../lciamethods/b2ad6494-c78d-11e6-9d9d-cec0c932ce01.xml"}, "other": {"anies": [{"name": "referenceToUnitGroupDataSet", "value": {"shortDescription": [{"value": "kg Sb eq", "lang": "en"}], "type": "unit group data set", "refObjectId": "54ccd2d9-a32a-4fc2-923d-f2c8c93e89d4", "uri": "../unitgroups/54ccd2d9-a32a-4fc2-923d-f2c8c93e89d4.xml"}}, {"value": "5.50820237855E-07", "module": "A1-A3"}, {"value": "9.46429544244766E-09", "module": "A4"}, {"value": "7.26029407601822E-10", "module": "A5"}, {"value": "0", "module": "C1"}, {"value": "4.21739355714774E-10", "module": "C2"}, {"value": "3.43634822174071E-08", "module": "C3"}, {"value": "0", "module": "C4"}, {"value": "-7.01391359046189E-08", "module": "D"}]}}, {"referenceToLCIAMethodDataSet": {"shortDescription": [{"value": "Abiotic depletion potential for fossil resources (ADPF)", "lang": "en"}, {"value": "Potenzial für den abiotischen Abbau fossiler Brennstoffe (ADPF)", "lang": "de"}], "type": "LCIA method data set", "refObjectId": "b2ad6110-c78d-11e6-9d9d-cec0c932ce01", "uri": "../lciamethods/b2ad6110-c78d-11e6-9d9d-cec0c932ce01.xml"}, "other": {"anies": [{"name": "referenceToUnitGroupDataSet", "value": {"shortDescription": [{"value": "MJ", "lang": "en"}], "type": "unit group data set", "refObjectId": "93a60a57-a3c8-11da-a746-0800200c9a66", "uri": "../unitgroups/93a60a57-a3c8-11da-a746-0800200c9a66.xml"}}, {"value": "49.0073433138169", "module": "A1-A3"}, {"value": "1.23265541069949", "module": "A4"}, {"value": "0.0767297338553534", "module": "A5"}, {"value": "0", "module": "C1"}, {"value": "0.0549284732168384", "module": "C2"}, {"value": "2.67735236961831", "module": "C3"}, {"value": "0", "module": "C4"}, {"value": "-4.67011683353068", "module": "D"}]}}, {"referenceToLCIAMethodDataSet": {"shortDescription": [{"value": "Water use (WDP)", "lang": "en"}, {"value": "Wassernutzung (WDP)", "lang": "de"}], "type": "LCIA method data set", "refObjectId": "b2ad66ce-c78d-11e6-9d9d-cec0c932ce01", "uri": "../lciamethods/b2ad66ce-c78d-11e6-9d9d-cec0c932ce01.xml"}, "other": {"anies": [{"name": "referenceToUnitGroupDataSet", "value": {"shortDescription": [{"value": "m^(3) world eq deprived", "lang": "en"}], "type": "unit group data set", "refObjectId": "6ae2df01-888e-46c8-b17d-49fa3869b476", "uri": "../unitgroups/6ae2df01-888e-46c8-b17d-49fa3869b476.xml"}}, {"value": "0.344720126068233", "module": "A1-A3"}, {"value": "0.00105059104214624", "module": "A4"}, {"value": "0.0300416842852769", "module": "A5"}, {"value": "0", "module": "C1"}, {"value": "4.68154858360888E-05", "module": "C2"}, {"value": "0.204590537116541", "module": "C3"}, {"value": "0", "module": "C4"}, {"value": "-0.0587088991708586", "module": "D"}]}}, {"referenceToLCIAMethodDataSet": {"shortDescription": [{"value": "Incidence of disease due to PM emissions (PM)", "lang": "en"}, {"value": "Auftreten von Krankheiten aufgrund von Feinstaubemissionen (PM)", "lang": "de"}], "type": "LCIA method data set", "refObjectId": "b5c602c6-def3-11e6-bf01-fe55135034f3", "uri": "../lciamethods/b5c602c6-def3-11e6-bf01-fe55135034f3.xml"}, "other": {"anies": [{"name": "referenceToUnitGroupDataSet", "value": {"shortDescription": [{"value": "Disease incidence", "lang": "en"}], "type": "unit group data set", "refObjectId": "3883559b-648f-4afc-8ba2-0bd24f3affa3", "uri": "../unitgroups/3883559b-648f-4afc-8ba2-0bd24f3affa3.xml"}}, {"value": "2.02104549738651E-07", "module": "A1-A3"}, {"value": "7.20979000558376E-10", "module": "A4"}, {"value": "2.51887740802337E-10", "module": "A5"}, {"value": "0", "module": "C1"}, {"value": "3.21276127767133E-11", "module": "C2"}, {"value": "1.02098807645752E-08", "module": "C3"}, {"value": "0", "module": "C4"}, {"value": "-5.33955365315766E-09", "module": "D"}]}}, {"referenceToLCIAMethodDataSet": {"shortDescription": [{"value": "Human exposure efficiency relative to U235 (IR)", "lang": "en"}, {"value": "Wirkung durch Exposition des Menschen mit U235 (IR)", "lang": "de"}], "type": "LCIA method data set", "refObjectId": "b5c632be-def3-11e6-bf01-fe55135034f3", "uri": "../lciamethods/b5c632be-def3-11e6-bf01-fe55135034f3.xml"}, "other": {"anies": [{"name": "referenceToUnitGroupDataSet", "value": {"shortDescription": [{"value": "kBq U235 eq", "lang": "en"}], "type": "unit group data set", "refObjectId": "456b05bf-1415-44a9-9993-02452f554c09", "uri": "../unitgroups/456b05bf-1415-44a9-9993-02452f554c09.xml"}}, {"value": "0.437836046616464", "module": "A1-A3"}, {"value": "0.000346869180978447", "module": "A4"}, {"value": "0.000598110859393173", "module": "A5"}, {"value": "0", "module": "C1"}, {"value": "1.54568700642051E-05", "module": "C2"}, {"value": "0.0105934799116906", "module": "C3"}, {"value": "0", "module": "C4"}, {"value": "-0.126491406394731", "module": "D"}]}}, {"referenceToLCIAMethodDataSet": {"shortDescription": [{"value": "Comparative toxic unit for ecosystems (ETP-fw)", "lang": "en"}, {"value": "Toxizitätsvergleichseinheit für Ökosysteme (ETP-fw)", "lang": "de"}], "type": "LCIA method data set", "refObjectId": "ee1082d1-b0f7-43ca-a1f0-21e2a4a74511", "uri": "../lciamethods/ee1082d1-b0f7-43ca-a1f0-21e2a4a74511.xml"}, "other": {"anies": [{"name": "referenceToUnitGroupDataSet", "value": {"shortDescription": [{"value": "CTUe", "lang": "en"}], "type": "unit group data set", "refObjectId": "aa959ded-f1eb-4efb-9c5c-2d60be36b3e6", "uri": "../unitgroups/aa959ded-f1eb-4efb-9c5c-2d60be36b3e6.xml"}}, {"value": "18.153467906129", "module": "A1-A3"}, {"value": "0.873511614121532", "module": "A4"}, {"value": "0.0411155099535461", "module": "A5"}, {"value": "0", "module": "C1"}, {"value": "0.0389246328571621", "module": "C2"}, {"value": "2.16249946336453", "module": "C3"}, {"value": "0", "module": "C4"}, {"value": "-2.04633371701105", "module": "D"}]}}, {"referenceToLCIAMethodDataSet": {"shortDescription": [{"value": "Comparative toxic unit for humans (carcinogenic) (HTP-c)", "lang": "en"}, {"value": "Toxizitätsvergleichseinheit für Menschen (krebserregend) (HTP-c)", "lang": "de"}], "type": "LCIA method data set", "refObjectId": "2299222a-bbd8-474f-9d4f-4dd1f18aea7c", "uri": "../lciamethods/2299222a-bbd8-474f-9d4f-4dd1f18aea7c.xml"}, "other": {"anies": [{"name": "referenceToUnitGroupDataSet", "value": {"shortDescription": [{"value": "CTUh", "lang": "en"}], "type": "unit group data set", "refObjectId": "d4c9523e-2d7e-49fd-8469-998f547d3a70", "uri": "../unitgroups/d4c9523e-2d7e-49fd-8469-998f547d3a70.xml"}}, {"value": "1.40374000560179E-09", "module": "A1-A3"}, {"value": "1.80061830927637E-11", "module": "A4"}, {"value": "2.38694403812018E-12", "module": "A5"}, {"value": "0", "module": "C1"}, {"value": "8.02375211404061E-13", "module": "C2"}, {"value": "8.77311444880313E-11", "module": "C3"}, {"value": "0", "module": "C4"}, {"value": "-8.2442069442509E-11", "module": "D"}]}}, {"referenceToLCIAMethodDataSet": {"shortDescription": [{"value": "Comparative toxic unit for humans (noncarcinogenic) (HTP-nc)", "lang": "en"}, {"value": "Toxizitätsvergleichseinheit für Menschen (nicht krebserregend) (HTP-nc)", "lang": "de"}], "type": "LCIA method data set", "refObjectId": "3af763a5-b7a1-48c9-9cee-1f223481fcef", "uri": "../lciamethods/3af763a5-b7a1-48c9-9cee-1f223481fcef.xml"}, "other": {"anies": [{"name": "referenceToUnitGroupDataSet", "value": {"shortDescription": [{"value": "CTUh", "lang": "en"}], "type": "unit group data set", "refObjectId": "d4c9523e-2d7e-49fd-8469-998f547d3a70", "uri": "../unitgroups/d4c9523e-2d7e-49fd-8469-998f547d3a70.xml"}}, {"value": "2.69220639663845E-08", "module": "A1-A3"}, {"value": "9.76800779134184E-10", "module": "A4"}, {"value": "1.36692754354711E-10", "module": "A5"}, {"value": "0", "module": "C1"}, {"value": "4.35273110142048E-11", "module": "C2"}, {"value": "8.9710216154221E-09", "module": "C3"}, {"value": "0", "module": "C4"}, {"value": "-2.22606827307151E-09", "module": "D"}]}}, {"referenceToLCIAMethodDataSet": {"shortDescription": [{"value": "Soil quality index (SQP)", "lang": "en"}, {"value": "Bodenqualitätsindex (SQP)", "lang": "de"}], "type": "LCIA method data set", "refObjectId": "b2ad6890-c78d-11e6-9d9d-cec0c932ce01", "uri": "../lciamethods/b2ad6890-c78d-11e6-9d9d-cec0c932ce01.xml"}, "other": {"anies": [{"name": "referenceToUnitGroupDataSet", "value": {"shortDescription": [{"value": "SQP", "lang": "en"}], "type": "unit group data set", "refObjectId": "f130951c-e67f-4f7f-8dd4-665de3974e18", "uri": "../unitgroups/f130951c-e67f-4f7f-8dd4-665de3974e18.xml"}}, {"value": "237.094936639611", "module": "A1-A3"}, {"value": "0.521786164411302", "module": "A4"}, {"value": "0.0228793948420187", "module": "A5"}, {"value": "0", "module": "C1"}, {"value": "0.0232513621471219", "module": "C2"}, {"value": "0.626327285140482", "module": "C3"}, {"value": "0", "module": "C4"}, {"value": "-1.68414885579182", "module": "D"}]}}]}, "otherAttributes": {"{http://www.indata.network/EPD/2019}epd-version": "1.2"}, "version": "1.1", "locations": "../ILCDLocations.xml"}