{"processInformation": {"dataSetInformation": {"UUID": "938c7bea-9acc-4237-94dc-accf28ae7b48", "name": {"baseName": [{"value": "RAUSIKKO Box", "lang": "de"}, {"value": "RAUSIKKO Box", "lang": "en"}], "functionalUnitFlowProperties": [{"lang": "de"}]}, "classificationInformation": {"classification": [{"class": [{"value": "Kunststoffe", "level": 0, "classId": "6"}, {"value": "Rohre", "level": 1, "classId": "6.1"}, {"value": "Regen-/Grauwasserrohre", "level": 2, "classId": "6.1.03"}], "name": "OEKOBAU.DAT"}, {"class": [{"value": "03 Gebäudetechnik", "level": 0}, {"value": "Anlagen zur Wasserversorgung und -entsorgung", "level": 1}, {"value": "Sickerboxen", "level": 2}], "name": "IBUCategories"}]}, "generalComment": [{"value": "Die EPD gilt fr die Sickerboxen bzw. die Elemente:\nRAUSIKKO Box 8.6 SC\nRAUSIKKO Box 8.3 SC\nRAUSIKKO Box 8.6 S\nRAUSIKKO Box 8.3 S\nRAUSIKKO Box Frontgitter\n\nRAUSIKKO Box SX, bestehend aus den Einzelelementen:\nRAUSIKKO Grundelement SX\nRAUSIKKO Deckplatte 8.3 SX\nRAUSIKKO Seitengitter 8.6 SX\nRAUSIKKO Seitengitter 8.3 SX\nRAUSIKKO Box MX, bestehend aus den Einzelelementen:\nRAUSIKKO Grundelement MX\nRAUSIKKO Deckplatte 8.3 MX\nRAUSIKKO Seitengitter 8.6 MX\nRAUSIKKO Seitengitter 8.3 MX\nRAUSIKKO Box LT, bestehend aus den Einzelelementen:\nRAUSIKKO Box LT Bodenplatte\nRAUSIKKO Box LT Grundelement\n\nBei den zu deklarierenden Sickerboxen handelt es sich um die Produktfamilie RAUSIKKO Box, die aus Polypropylen (PP) bestehen. Bei der Mehrheit der Elemente wird PP aus zugekauftem Post-Industrial-Rezyklat (PIR) verwendet, bei einem geringeren Anteil auch PP aus Neuware.", "lang": "de"}, {"value": "The EPD applies to the infiltration boxes and the elements\nRAUSIKKO Box 8.6 SC\nRAUSIKKO Box 8.3 SC\nRAUSIKKO Box 8.6 S\nRAUSIKKO Box 8.3 S\nRAUSIKKO Box front grille\n\nRAUSIKKO Box SX, consisting of the individual elements:\nRAUSIKKO Basic element SX\nRAUSIKKO Cover plate 8.3 SX\nRAUSIKKO Side rail 8.6 SX\nRAUSIKKO Side rail 8.3 SX\n\nRAUSIKKO Box MX, consisting of the individual elements:\nRAUSIKKO Basic element MX\nRAUSIKKO Cover plate 8.3 MX\nRAUSIKKO Side rail 8.6 MX\nRAUSIKKO Side rail 8.3 MX\n\nRAUSIKKO Box LT, consisting of the individual elements:\nRAUSIKKO Box LT Base plate\nRAUSIKKO Box LT Basic element\nThe infiltration boxes to be declared are from the RAUSIKKO Box product family, which are made of polypropylene (PP). For the majority of the elements, PP from purchased post-industrial recyclate (PIR) is used, while a smaller proportion uses PP from virgin material.", "lang": "en"}], "other": {"anies": [{"scenario": [{"description": [{"value": "100 % stoffliche Verwertung der Sickerboxen (EoLSzenario 1, C3 und C4)", "lang": "de"}, {"value": "100 % material recycling (EoL scenario 1, C3 and C4)", "lang": "en"}], "name": "S0", "default": true}, {"description": [{"value": "100 % energetische Verwertung (EoL-Szenario 2, C3/1 und C4/1)", "lang": "de"}, {"value": "100 % energy recovery (EoL scenario 2, C3/1 and C4/1)", "lang": "en"}], "name": "S1"}, {"description": [{"value": "100 % Deponierung der Sickerboxen (EoL-Szenario 3, C3/2 und C4/2)", "lang": "de"}, {"value": "100 % landfilling of the infiltration boxes (EoL scenario 3, C3/2 and C4/2)", "lang": "en"}], "name": "S2"}]}]}}, "quantitativeReference": {"referenceToReferenceFlow": [0]}, "time": {"referenceYear": 2025, "dataSetValidUntil": 2030, "other": {"anies": [{"name": "publicationDateOfEPD", "value": 1746144000000}]}}, "geography": {"locationOfOperationSupplyOrProduction": {"location": "RER"}}, "technology": {"technologyDescriptionAndIncludedProcesses": [{"value": "Bei den zu deklarierenden Sickerboxen handelt es sich um die Produktfamilie RAUSIKKO Box, die aus Polypropylen (PP) bestehen. Bei der Mehrheit der Elemente wird PP aus zugekauftem Post-Industrial-Rezyklat (PIR) verwendet, bei einem geringeren Anteil auch PP aus Neuware. Die Elemente der RAUSIKKO Boxen werden im Spritzgussverfahren hergestellt. Die Sickerboxen werden allgemein für die Speicherung, Versickerung und Rückhaltung von Regenwasser eingesetzt. Die Boxen können als Box- und Mulden-Box-Rigolen aufgebaut werden. Sie sind einsetzbar an Wohn- und Gewerbebauten, auf Logistikflächen und Parkplätzen sowie an Straßen und in Erschließungsgebieten. \nTechnische Daten: \nDie technischen Daten der Produkte, die im Geltungsbereich der EPD liegen, sind unter Verweis auf die den einzelnen Daten zugrundeliegenden Prfregeln genannt.\nDie Leistungswerte des Produkts in Bezug auf dessen Merkmale gelten nach der magebenden technischen Bestimmung (DIN EN 17152-1). \nDeklarierte Einheit: \nAls deklarierte Einheit wird \"1 kg Sickerbox ohne Produktverpackung\" verwendet. Die Produktverpackung wird separat zum Produkt betrachtet und ist ebenfalls Teil der kobilanz.\n\nFr die LCA wurde eine Durchschnittsvariante der Sickerbox RAUSIKKO Box bilanziert. Diese basiert auf den produzierten Tonnagen fr das Produktionsjahr 2022 bzw. 2023 und deckt damit alle Produktvarianten (gelistet in 2.1) ab. Der zugehrige Massebezug unterscheidet sich je nach Produktsystem und betrachtetem Element und kann in den Technischen Daten nachgeschlagen werden.", "lang": "de"}, {"value": "The infiltration boxes to be declared are from the RAUSIKKO Box product family, which are made of polypropylene (PP). PP from purchased post-industrial recyclate (PIR) is used for the majority of the elements, and PP from virgin material is also used for a smaller proportion. The elements of the RAUSIKKO boxes are manufactured by injection moulding. The infiltration boxes are generally used for the storage, infiltration and retention of rainwater. The boxes can be constructed as box and trough box infiltration systems. They can be used in residential and commercial buildings, on logistics areas and car parks as well as on roads and in development areas. \nTechnical data: \nThe technical data of the products within the scope of the EPD are provided with reference to the testing rules on which the individual data are based.\n\nThe performance values of the product in relation to its characteristics apply according to the relevant technical regulation (DIN EN 17152-1). \nDeclared unit: \nThe declared unit is \"1 kg infiltration box without product packaging\". The product packaging is considered separately from the product and is also included in the LCA. \n\nFor the LCA, an average variant of the infiltration box RAUSIKKO Box is used. This is based on the produced tonnages for the production year 2022 or 2023 and thus covers all product variants (listed in 2.1). The associated mass reference varies depending on the product system and element under consideration and can be found in the technical data.", "lang": "en"}], "technologicalApplicability": [{"value": "Die Sickerboxen werden allgemein fr die Speicherung, Versickerung und Rckhaltung von Regenwasser eingesetzt. Die Boxen knnen als Box- und Mulden-Box-Rigolen aufgebaut werden. Sie sind einsetzbar an Wohn- und Gewerbebauten, auf Logistikflchen und Parkpltzen sowie an Straen und in Erschlieungsgebieten.", "lang": "de"}, {"value": "Infiltration boxes are generally used for the storage, infiltration, and retention of rainwater. The boxes can be configured as box and trough box infiltration systems. They are suitable for use in residential and commercial buildings, logistics areas, parking lots, as well as on roads and in development areas.", "lang": "en"}]}}, "modellingAndValidation": {"LCIMethodAndAllocation": {"typeOfDataSet": "EPD", "referenceToLCAMethodDetails": [{"shortDescription": [{"value": "Sickerboxen.pdf", "lang": "de"}], "type": "source data set", "refObjectId": "153eeb02-4891-4922-9e19-3755f420e2c4"}], "other": {"anies": [{"name": "subType", "value": "average dataset"}]}}, "dataSourcesTreatmentAndRepresentativeness": {"referenceToDataSource": [{"shortDescription": [{"value": "GaBi Database (all versions)", "lang": "de"}], "type": "source data set", "refObjectId": "28d74cc0-db8b-4d7e-bc44-5f6d56ce0c4a"}, {"shortDescription": [{"value": "Sphera MLC (fka GaBi) Databases Edition 2024", "lang": "de"}], "type": "source data set", "refObjectId": "7443b962-0446-4d69-8aa7-8055a6b1614a"}], "useAdviceForDataSet": [{"value": "Gültigkeitsbereich: \nDie EPD gilt fr die Sickerboxen bzw. die Elemente\nRAUSIKKO Box 8.6 SC\nRAUSIKKO Box 8.3 SC\nRAUSIKKO Box 8.6 S\nRAUSIKKO Box 8.3 S\nRAUSIKKO Box Frontgitter\nRAUSIKKO Box SX, bestehend aus den Einzelelementen:\n\nRAUSIKKO Grundelement SX\nRAUSIKKO Deckplatte 8.3 SX\nRAUSIKKO Seitengitter 8.6 SX\nRAUSIKKO Seitengitter 8.3 SX\n\nRAUSIKKO Box MX, bestehend aus den Einzelelementen:\nRAUSIKKO Grundelement MX\nRAUSIKKO Deckplatte 8.3 MX\nRAUSIKKO Seitengitter 8.6 MX\nRAUSIKKO Seitengitter 8.3 MX\n\nRAUSIKKO Box LT, bestehend aus den Einzelelementen:\n\nRAUSIKKO Box LT Bodenplatte\n\nRAUSIKKO Box LT Grundelement\nhergestellt im\nREHAU-Werk Viechtach, Deutschland\nder Firma\nREHAU Industries SE & Co. KG.\nDie Herstellung der Sickerboxen erfolgt vor allem in Deutschland und teilweise im europischen Ausland. Die Produkte werden weltweit verwendet, mit dem Fokus auf Europa. Es handelt sich um eine Durchschnitts-EPD, bei der die oben genannten Produkte ber eine durchschnittliche Produktvariante deklariert werden. \nSystemgrenze: \nEs wird der gesamte Produktlebenszyklus von RAUSIKKO Box betrachtet – siehe Flieschema. Typ der EPD: Wiege bis Bahre (Module A, B, C, D).\n\nDas nachfolgende Flieschema zeigt die Systemgrenzen bei der Bilanzierung von RAUSIKKO Box:\n\n\nIm Folgenden sind die bercksichtigten Lebenswegabschnitte bzw. Prozessmodule der Sickerboxen detailliert aufgelistet:\n\nA1 – A3 Herstellungsphase\nProduktion der Roh-, Hilfs- und Betriebsstoffe inkl. Transport zum jeweiligen Werk\nRegranulierung des Input-Mahlguts zu Regranulat inkl. Transport zum jeweiligen Werk\nProduktion der Verpackungsmaterialien fr das Endprodukt\nEnergiebereitstellung fr die Produktion\nProduktion und Verpackung der Sickerboxen im jeweiligen Werk\nProduktion der Verpackungsmaterialien der Rohstoffe inkl. Transporte zur Verwertung mit anschlieender Verwertung\nInterne Wiederaufbereitung der Produktionsabflle zum Mahlgut\nA4 – A5 Bauphase\nTransport des Produkts zur Baustelle\nVerlegung der Sickerbox auf der Baustelle\nVerwertung der Produktverpackung\nB Nutzungsphase\nNutzung der Sickerboxen (B1)\nInstandhaltung durch Wassersplung der Sickerboxen (B2)\nBetrieblicher Energie- und Wassereinsatz (B6, B7)\nC1 – C4 Entsorgung\nEs werden drei 100 %-Entsorgungsszenarien angenommen:\nEnd-of-Life (EoL)-Szenario 1 (Recycling): 100 % Rckbau der Sickerboxen mittels Bagger inkl. Transport zum Ort der Verwertung mit werkstofflicher Verwertung (Module C3, C4 und D in der Auswertung).\nEoL-Szenario 2 (Energierckgewinnung aus Abfllen): 100 % Rckbau der Sickerboxen mittels Bagger inkl. Transport zum Ort der Verwertung mit Energierckgewinnung (Module C3/1, C4/1 und D/1 in der Auswertung).\nEoL-Szenario 3 (Deponierung): 100 % Rckbau der Sickerboxen mittels Bagger inkl. Transport zum Ort der Entsorgung. Die Entsorgung findet auf einer lokalen Deponie statt (Module C3/2, C4/2 und D/2 in der Auswertung).\nD Wiederverwendungs-, Rckgewinnungs- und/oder Recyclingpotentiale\nWiederverwendungs-, Rckgewinnungs-, und/oder Recyclingpotentiale sind in den Entsorgungsszenarien vorhanden, da hier die Sickerboxen einer energetischen bzw. stofflichen Verwertung zugefhrt werden, aus der Energie bzw. Sekundrmaterialien zurckgewonnen wird, die auerhalb der Systemgrenze genutzt werden knnen. Auerdem entstehen anrechenbare Potentiale durch die Verwertung der Produktverpackung in Modul A5.", "lang": "de"}, {"value": "Scope: \nThe EPD applies to the infiltration boxes and the elements\nRAUSIKKO Box 8.6 SC\nRAUSIKKO Box 8.3 SC\nRAUSIKKO Box 8.6 S\nRAUSIKKO Box 8.3 S\nRAUSIKKO Box front grille\nRAUSIKKO Box SX, consisting of the individual elements:\nRAUSIKKO Basic element SX\nRAUSIKKO Cover plate 8.3 SX\nRAUSIKKO Side rail 8.6 SX\nRAUSIKKO Side rail 8.3 SX\n\nRAUSIKKO Box MX, consisting of the individual elements:\nRAUSIKKO Basic element MX\nRAUSIKKO Cover plate 8.3 MX\nRAUSIKKO Side rail 8.6 MX\nRAUSIKKO Side rail 8.3 MX\n\nRAUSIKKO Box LT, consisting of the individual elements:\nRAUSIKKO Box LT Base plate\nRAUSIKKO Box LT Basic element\n\nmanufactured in\nREHAU plant Viechtach, Germany\n\nof the company\nREHAU Industries SE & Co KG.\n\nThe infiltration boxes are manufactured mainly in Germany and partly in other European countries. The products are used worldwide, with a focus on Europe. This is an average EPD in which the above-mentioned products are declared via an average product variant. \nSystem boundary: \nThe entire product life cycle of RAUSIKKO Box is considered - see flow chart. \nType of EPD: cradle to grave (modules A, B, C, D). \n\nThe following flow diagram shows the system limits when balancing RAUSIKKO Box:\n\n\nThe following is a detailed list of the life cycle stages and process modules considered for the infiltration boxes:\n\nA1 - A3 Production phase\nProduction of raw materials, supplies, and operating materials, including transport to the respective plant\nRegranulation of the input regrind into regranulate, including transport to the respective plant\nProduction of packaging materials for the end product\nEnergy supply for production\nProduction and packaging of the infiltration boxes at the respective plant\nProduction of packaging materials for raw materials, including transport for recycling and subsequent utilisation\nInternal reprocessing of production waste into regrind\nA4 - A5 Construction phase\nTransport of the product to the construction site\nInstallation of the infiltration box on the construction site\nRecycling of product packaging\nB Utilisation phase\nUtilisation of the infiltration boxes (B1)\nMaintenance through water flushing of the infiltration boxes (B2)\nOperational energy and water use (B6, B7)\n\nC1 - C4 Disposal\nThree 100 % disposal scenarios are assumed:\nEnd-of-life (EoL) scenario 1 (recycling): 100 % dismantling of the infiltration boxes using an excavator, including transport to the recycling site with material recycling (modules C3, C4 and D in the evaluation).\nEoL scenario 2 (energy recovery from waste): 100 % dismantling of the infiltration boxes using an excavator incl. transport to the recycling site with Energy recovery (modules C3/1, C4/1 and D/1 in the evaluation).\nEoL scenario 3 (landfill): 100 % dismantling of the infiltration boxes using an excavator, including transport to the disposal site. Disposal takes place at a local landfill (modules C3/2, C4/2 and D/2 in the evaluation). \nD Potential for reuse, recovery and/or recycling \nThere is potential for reuse, recovery, and/or recycling in the disposal scenarios, as the infiltration boxes are subjected to energy or material recovery processes, from which energy or secondary materials that can be utilized outside the system boundary are recovered. Additionally, creditable potentials arise from the recycling of product packaging in Module A5.", "lang": "en"}], "other": {"anies": [{"name": "referenceToOriginalEPD", "value": {"shortDescription": {"value": "RAUSIKKO Box.pdf", "defaultValue": "RAUSIKKO Box.pdf", "lstrings": [{"lang": "de", "value": "RAUSIKKO Box.pdf"}]}, "type": "source data set", "uuid": {"uuid": "e0435f16-bb13-4bd0-8635-5993752da6d3"}, "refObjectId": "e0435f16-bb13-4bd0-8635-5993752da6d3", "resourceURLs": ["https://oekobaudat.de/OEKOBAU.DAT/resource/sources/e0435f16-bb13-4bd0-8635-5993752da6d3/RAUSIKKO_Box_20739.pdf?version=00.01.000"]}}]}}, "validation": {"review": [{"referenceToNameOfReviewerAndInstitution": [{"shortDescription": [{"value": "Institut Bauen und Umwelt e. V.", "lang": "de"}], "type": "contact data set", "refObjectId": "d111dbec-b024-4be5-86c5-752d6eb2cf95", "uri": "../contacts/d111dbec-b024-4be5-86c5-752d6eb2cf95.xml"}], "type": "Accredited third party review"}]}, "complianceDeclarations": {"compliance": [{"referenceToComplianceSystem": {"shortDescription": [{"value": "DIN EN 15804+A2", "lang": "de"}], "type": "source data set", "refObjectId": "c0016b33-8cf7-415c-ac6e-deba0d21440d", "uri": "../sources/c0016b33-8cf7-415c-ac6e-deba0d21440d.xml"}}, {"referenceToComplianceSystem": {"shortDescription": [{"value": "ISO 14025", "lang": "de"}], "type": "source data set", "refObjectId": "4f2eb655-6e44-4874-a95a-e28f5442cd4d", "uri": "../sources/4f2eb655-6e44-4874-a95a-e28f5442cd4d.xml"}}]}}, "administrativeInformation": {"commissionerAndGoal": {"referenceToCommissioner": [{"shortDescription": [{"value": "REHAU Industries SE & Co. KG", "lang": "de"}], "type": "contact data set", "refObjectId": "b1b59d51-66a3-4983-acd8-86ad04e48050", "uri": "../contacts/b1b59d51-66a3-4983-acd8-86ad04e48050.xml"}]}, "dataGenerator": {"referenceToPersonOrEntityGeneratingTheDataSet": [{"shortDescription": [{"value": "SKZ - Das Kunststoff-Zentrum", "lang": "de"}], "type": "contact data set", "refObjectId": "2da43b2d-777d-45c6-ba4b-76c55a616a00", "uri": "../contacts/2da43b2d-777d-45c6-ba4b-76c55a616a00.xml"}]}, "dataEntryBy": {"timeStamp": 1746144000000, "referenceToDataSetFormat": [{"shortDescription": [{"value": "ILCD Format", "lang": "de"}], "type": "source data set", "refObjectId": "a97a0155-0234-4b87-b4ce-a45da52f2a40", "uri": "../sources/a97a0155-0234-4b87-b4ce-a45da52f2a40.xml"}, {"shortDescription": [{"value": "EPD-Datenformaterweiterungen v1.2", "lang": "de"}, {"value": "EPD Data Format Extensions v1.2", "lang": "en"}], "type": "source data set", "refObjectId": "a29449fd-aa2f-4de8-b5d7-4b06b43c6fde", "uri": "../sources/a29449fd-aa2f-4de8-b5d7-4b06b43c6fde.xml"}]}, "publicationAndOwnership": {"dataSetVersion": "00.01.000", "referenceToRegistrationAuthority": {"shortDescription": [{"value": "Institut Bauen und Umwelt e. V.", "lang": "de"}], "type": "contact data set", "refObjectId": "d111dbec-b024-4be5-86c5-752d6eb2cf95", "uri": "../contacts/d111dbec-b024-4be5-86c5-752d6eb2cf95.xml"}, "registrationNumber": "EPD-REH-20250008-IBC1-DE", "referenceToOwnershipOfDataSet": {"shortDescription": [{"value": "REHAU Industries SE & Co. KG", "lang": "de"}], "type": "contact data set", "refObjectId": "b1b59d51-66a3-4983-acd8-86ad04e48050", "uri": "../contacts/b1b59d51-66a3-4983-acd8-86ad04e48050.xml"}, "copyright": true, "licenseType": "Free of charge for all users and uses", "accessRestrictions": [{"value": "None", "lang": "en"}], "other": {"anies": [{"name": "referenceToPublisher", "value": {"shortDescription": [{"value": "Institut Bauen und Umwelt e. V.", "lang": "de"}], "type": "contact data set", "refObjectId": "d111dbec-b024-4be5-86c5-752d6eb2cf95", "uri": "../contacts/d111dbec-b024-4be5-86c5-752d6eb2cf95.xml"}}]}}}, "exchanges": {"exchange": [{"dataSetInternalID": 0, "referenceToFlowDataSet": {"shortDescription": [{"value": "RAUSIKKO Box (Sickerbox)", "lang": "de"}], "type": "flow data set", "refObjectId": "76c7631e-167a-6ea3-9e24-74da60bb6ed6", "uri": "../flows/76c7631e-167a-6ea3-9e24-74da60bb6ed6.xml"}, "meanAmount": 1.0, "referencesToDataSource": {}, "referenceFlow": true, "resolvedFlowVersion": "00.01.000", "resultingflowAmount": 1.0, "flowProperties": [{"name": [{"lang": "en", "value": "Mass"}, {"lang": "de", "value": "Masse"}], "uuid": "93a60a56-a3c8-11da-a746-0800200b9a66", "referenceFlowProperty": true, "meanValue": 1.0, "referenceUnit": "kg", "unitGroupUUID": "ad38d542-3fe9-439d-9b95-2f5f7752acaf"}], "materialProperties": [{"name": "gross density", "value": "900.0", "unit": "kg/m^3", "unitDescription": "kilograms per cubic metre"}], "typeOfFlow": "Product flow", "classification": {"classHierarchy": "Kunststoffe / Rohre / Regen-/Grauwasserrohre", "name": "OEKOBAU.DAT"}}, {"dataSetInternalID": 1, "referenceToFlowDataSet": {"shortDescription": [{"value": "Erneuerbare Primärenergie als Energieträger (PERE)", "lang": "de"}, {"value": "Renewable primary energy as energy carrier (PERE)", "lang": "en"}], "type": "flow data set", "refObjectId": "20f32be5-0398-4288-9b6d-accddd195317", "uri": "../flows/20f32be5-0398-4288-9b6d-accddd195317.xml"}, "exchange direction": "INPUT", "other": {"anies": [{"name": "referenceToUnitGroupDataSet", "value": {"shortDescription": [{"value": "MJ", "lang": "de"}], "type": "unit group data set", "refObjectId": "93a60a57-a3c8-11da-a746-0800200c9a66", "uri": "../unitgroups/93a60a57-a3c8-11da-a746-0800200c9a66.xml"}}, {"value": "9.51360869510847", "module": "A1-A3"}, {"value": "0.0473112205006587", "module": "A4"}, {"value": "0.500835367981233", "module": "A5"}, {"value": "0", "module": "B1"}, {"value": "0.0158410925634753", "module": "B2"}, {"value": "0", "module": "B6"}, {"value": "0", "module": "B7"}, {"value": "0.0646749163957641", "module": "C1"}, {"value": "0.00763123358234849", "module": "C2"}, {"value": "0.0914187555674422", "module": "C3", "scenario": "S0"}, {"value": "0.106121205190906", "module": "C3", "scenario": "S1"}, {"value": "0.00127907400052268", "module": "C3", "scenario": "S2"}, {"value": "0", "module": "C4", "scenario": "S0"}, {"value": "0", "module": "C4", "scenario": "S1"}, {"value": "0.075076348104652", "module": "C4", "scenario": "S2"}, {"value": "-0.265525868116098", "module": "D", "scenario": "S0"}, {"value": "-8.18091242377404", "module": "D", "scenario": "S1"}, {"value": "-0.103055836316208", "module": "D", "scenario": "S2"}]}, "resolvedFlowVersion": "38.00.000", "flowProperties": [], "typeOfFlow": "Other flow", "classification": {"classHierarchy": "Quantities", "name": "GaBiCategories"}}, {"dataSetInternalID": 2, "referenceToFlowDataSet": {"shortDescription": [{"value": "Erneuerbare Primärenergie zur stofflichen Nutzung (PERM)", "lang": "de"}, {"value": "Renewable primary energy resources as material utilization (PERM)", "lang": "en"}], "type": "flow data set", "refObjectId": "fb3ec0de-548d-4508-aea5-00b73bf6f702", "uri": "../flows/fb3ec0de-548d-4508-aea5-00b73bf6f702.xml"}, "exchange direction": "INPUT", "other": {"anies": [{"name": "referenceToUnitGroupDataSet", "value": {"shortDescription": [{"value": "MJ", "lang": "de"}], "type": "unit group data set", "refObjectId": "93a60a57-a3c8-11da-a746-0800200c9a66", "uri": "../unitgroups/93a60a57-a3c8-11da-a746-0800200c9a66.xml"}}, {"value": "0", "module": "A1-A3"}, {"value": "0", "module": "A4"}, {"value": "0", "module": "A5"}, {"value": "0", "module": "B1"}, {"value": "0", "module": "B2"}, {"value": "0", "module": "B6"}, {"value": "0", "module": "B7"}, {"value": "0", "module": "C1"}, {"value": "0", "module": "C2"}, {"value": "0", "module": "C3", "scenario": "S0"}, {"value": "0", "module": "C3", "scenario": "S1"}, {"value": "0", "module": "C3", "scenario": "S2"}, {"value": "0", "module": "C4", "scenario": "S0"}, {"value": "0", "module": "C4", "scenario": "S1"}, {"value": "0", "module": "C4", "scenario": "S2"}, {"value": "0", "module": "D", "scenario": "S0"}, {"value": "0", "module": "D", "scenario": "S1"}, {"value": "0", "module": "D", "scenario": "S2"}]}, "resolvedFlowVersion": "38.00.000", "flowProperties": [], "typeOfFlow": "Other flow", "classification": {"classHierarchy": "Quantities", "name": "GaBiCategories"}}, {"dataSetInternalID": 3, "referenceToFlowDataSet": {"shortDescription": [{"value": "Total erneuerbare Primärenergie (PERT)", "lang": "de"}, {"value": "Total use of renewable primary energy resources (PERT)", "lang": "en"}], "type": "flow data set", "refObjectId": "53f97275-fa8a-4cdd-9024-65936002acd0", "uri": "../flows/53f97275-fa8a-4cdd-9024-65936002acd0.xml"}, "exchange direction": "INPUT", "other": {"anies": [{"name": "referenceToUnitGroupDataSet", "value": {"shortDescription": [{"value": "MJ", "lang": "de"}], "type": "unit group data set", "refObjectId": "93a60a57-a3c8-11da-a746-0800200c9a66", "uri": "../unitgroups/93a60a57-a3c8-11da-a746-0800200c9a66.xml"}}, {"value": "9.51360869510847", "module": "A1-A3"}, {"value": "0.0473112205006587", "module": "A4"}, {"value": "0.500835367981233", "module": "A5"}, {"value": "0", "module": "B1"}, {"value": "0.0158410925634753", "module": "B2"}, {"value": "0", "module": "B6"}, {"value": "0", "module": "B7"}, {"value": "0.0646749163957641", "module": "C1"}, {"value": "0.00763123358234849", "module": "C2"}, {"value": "0.0914187555674422", "module": "C3", "scenario": "S0"}, {"value": "0.106121205190906", "module": "C3", "scenario": "S1"}, {"value": "0.00127907400052268", "module": "C3", "scenario": "S2"}, {"value": "0", "module": "C4", "scenario": "S0"}, {"value": "0", "module": "C4", "scenario": "S1"}, {"value": "0.075076348104652", "module": "C4", "scenario": "S2"}, {"value": "-0.265525868116098", "module": "D", "scenario": "S0"}, {"value": "0.765015482656563", "module": "D", "scenario": "S1"}, {"value": "-1.48821303185168E-10", "module": "D", "scenario": "S2"}]}, "resolvedFlowVersion": "38.00.000", "flowProperties": [], "typeOfFlow": "Other flow", "classification": {"classHierarchy": "Quantities / Environmental quantities / EPD EN 15804 / LCI indicators", "name": "GaBiCategories"}}, {"dataSetInternalID": 4, "referenceToFlowDataSet": {"shortDescription": [{"value": "Nicht-erneuerbare Primärenergie als Energieträger (PENRE)", "lang": "de"}, {"value": "Non renewable primary energy as energy carrier (PENRE)", "lang": "en"}], "type": "flow data set", "refObjectId": "ac857178-2b45-46ec-892a-a9a4332f0372", "uri": "../flows/ac857178-2b45-46ec-892a-a9a4332f0372.xml"}, "exchange direction": "INPUT", "other": {"anies": [{"name": "referenceToUnitGroupDataSet", "value": {"shortDescription": [{"value": "MJ", "lang": "de"}], "type": "unit group data set", "refObjectId": "93a60a57-a3c8-11da-a746-0800200c9a66", "uri": "../unitgroups/93a60a57-a3c8-11da-a746-0800200c9a66.xml"}}, {"value": "12.7518766292384", "module": "A1-A3"}, {"value": "0.549306578519644", "module": "A4"}, {"value": "5.16493942595684", "module": "A5"}, {"value": "0", "module": "B1"}, {"value": "0.180976215437602", "module": "B2"}, {"value": "0", "module": "B6"}, {"value": "0", "module": "B7"}, {"value": "0.765015499177783", "module": "C1"}, {"value": "0.0886023815205886", "module": "C2"}, {"value": "2.84083284238803", "module": "C3", "scenario": "S0"}, {"value": "3.66004049298064", "module": "C3", "scenario": "S1"}, {"value": "0.529013103649441", "module": "C3", "scenario": "S2"}, {"value": "0", "module": "C4", "scenario": "S0"}, {"value": "0", "module": "C4", "scenario": "S1"}, {"value": "0.496539709668982", "module": "C4", "scenario": "S2"}, {"value": "-2.24695077659658", "module": "D", "scenario": "S0"}, {"value": "-24.5765313370475", "module": "D", "scenario": "S1"}, {"value": "-0.309652389728497", "module": "D", "scenario": "S2"}]}, "resolvedFlowVersion": "38.00.000", "flowProperties": [], "typeOfFlow": "Other flow", "classification": {"classHierarchy": "Quantities", "name": "GaBiCategories"}}, {"dataSetInternalID": 5, "referenceToFlowDataSet": {"shortDescription": [{"value": "Nicht-erneuerbare Primärenergie zur stofflichen Nutzung (PENRM)", "lang": "de"}, {"value": "Non renewable primary energy as material utilization (PENRM)", "lang": "en"}], "type": "flow data set", "refObjectId": "1421caa0-679d-4bf4-b282-0eb850ccae27", "uri": "../flows/1421caa0-679d-4bf4-b282-0eb850ccae27.xml"}, "exchange direction": "INPUT", "other": {"anies": [{"name": "referenceToUnitGroupDataSet", "value": {"shortDescription": [{"value": "MJ", "lang": "de"}], "type": "unit group data set", "refObjectId": "93a60a57-a3c8-11da-a746-0800200c9a66", "uri": "../unitgroups/93a60a57-a3c8-11da-a746-0800200c9a66.xml"}}, {"value": "2.81826296065585", "module": "A1-A3"}, {"value": "0", "module": "A4"}, {"value": "0.475853966191159", "module": "A5"}, {"value": "0", "module": "B1"}, {"value": "0", "module": "B2"}, {"value": "0", "module": "B6"}, {"value": "0", "module": "B7"}, {"value": "0", "module": "C1"}, {"value": "0", "module": "C2"}, {"value": "-3.293897582", "module": "C3", "scenario": "S0"}, {"value": "-3.293897582", "module": "C3", "scenario": "S1"}, {"value": "-0.5246", "module": "C3", "scenario": "S2"}, {"value": "0", "module": "C4", "scenario": "S0"}, {"value": "0", "module": "C4", "scenario": "S1"}, {"value": "0", "module": "C4", "scenario": "S2"}, {"value": "0", "module": "D", "scenario": "S0"}, {"value": "0", "module": "D", "scenario": "S1"}, {"value": "0", "module": "D", "scenario": "S2"}]}, "resolvedFlowVersion": "38.00.000", "flowProperties": [], "typeOfFlow": "Other flow", "classification": {"classHierarchy": "Quantities", "name": "GaBiCategories"}}, {"dataSetInternalID": 6, "referenceToFlowDataSet": {"shortDescription": [{"value": "Total nicht erneuerbare Primärenergie (PENRT)", "lang": "de"}, {"value": "Total use of non renewable primary energy resources (PENRT)", "lang": "en"}], "type": "flow data set", "refObjectId": "06159210-646b-4c8d-8583-da9b3b95a6c1", "uri": "../flows/06159210-646b-4c8d-8583-da9b3b95a6c1.xml"}, "exchange direction": "INPUT", "other": {"anies": [{"name": "referenceToUnitGroupDataSet", "value": {"shortDescription": [{"value": "MJ", "lang": "de"}], "type": "unit group data set", "refObjectId": "93a60a57-a3c8-11da-a746-0800200c9a66", "uri": "../unitgroups/93a60a57-a3c8-11da-a746-0800200c9a66.xml"}}, {"value": "15.5701395898943", "module": "A1-A3"}, {"value": "0.549306578519644", "module": "A4"}, {"value": "5.640793392148", "module": "A5"}, {"value": "0", "module": "B1"}, {"value": "0.180976215437602", "module": "B2"}, {"value": "0", "module": "B6"}, {"value": "0", "module": "B7"}, {"value": "0.765015499177783", "module": "C1"}, {"value": "0.0886023815205886", "module": "C2"}, {"value": "-0.45306473961197", "module": "C3", "scenario": "S0"}, {"value": "0.36614291098064", "module": "C3", "scenario": "S1"}, {"value": "0.00441310364944103", "module": "C3", "scenario": "S2"}, {"value": "0", "module": "C4", "scenario": "S0"}, {"value": "0", "module": "C4", "scenario": "S1"}, {"value": "0.496539709668982", "module": "C4", "scenario": "S2"}, {"value": "-2.24695077659658", "module": "D", "scenario": "S0"}, {"value": "-24.5765313370475", "module": "D", "scenario": "S1"}, {"value": "-0.309652389728497", "module": "D", "scenario": "S2"}]}, "resolvedFlowVersion": "38.00.000", "flowProperties": [], "typeOfFlow": "Other flow", "classification": {"classHierarchy": "Quantities / Environmental quantities / EPD EN 15804 / LCI indicators", "name": "GaBiCategories"}}, {"dataSetInternalID": 7, "referenceToFlowDataSet": {"shortDescription": [{"value": "Einsatz von Sekundärstoffen (SM)", "lang": "de"}, {"value": "Use of secondary material (SM)", "lang": "en"}], "type": "flow data set", "refObjectId": "c6a1f35f-2d09-4f54-8dfb-97e502e1ce92", "uri": "../flows/c6a1f35f-2d09-4f54-8dfb-97e502e1ce92.xml"}, "exchange direction": "INPUT", "other": {"anies": [{"name": "referenceToUnitGroupDataSet", "value": {"shortDescription": [{"value": "kg", "lang": "de"}], "type": "unit group data set", "refObjectId": "ad38d542-3fe9-439d-9b95-2f5f7752acaf", "uri": "../unitgroups/ad38d542-3fe9-439d-9b95-2f5f7752acaf.xml"}}, {"value": "0.922643759623516", "module": "A1-A3"}, {"value": "0", "module": "A4"}, {"value": "0", "module": "A5"}, {"value": "0", "module": "B1"}, {"value": "0", "module": "B2"}, {"value": "0", "module": "B6"}, {"value": "0", "module": "B7"}, {"value": "0", "module": "C1"}, {"value": "0", "module": "C2"}, {"value": "0", "module": "C3", "scenario": "S0"}, {"value": "0", "module": "C3", "scenario": "S1"}, {"value": "0", "module": "C3", "scenario": "S2"}, {"value": "0", "module": "C4", "scenario": "S0"}, {"value": "0", "module": "C4", "scenario": "S1"}, {"value": "0", "module": "C4", "scenario": "S2"}, {"value": "0.028", "module": "D", "scenario": "S0"}, {"value": "0", "module": "D", "scenario": "S1"}, {"value": "0", "module": "D", "scenario": "S2"}]}, "resolvedFlowVersion": "38.00.000", "flowProperties": [], "typeOfFlow": "Other flow", "classification": {"classHierarchy": "Quantities / Environmental quantities / EPD EN 15804 / LCI indicators", "name": "GaBiCategories"}}, {"dataSetInternalID": 8, "referenceToFlowDataSet": {"shortDescription": [{"value": "Erneuerbare Sekundärbrennstoffe (RSF)", "lang": "de"}, {"value": "Use of renewable secondary fuels (RSF)", "lang": "en"}], "type": "flow data set", "refObjectId": "64333088-a55f-4aa2-9a31-c10b07816787", "uri": "../flows/64333088-a55f-4aa2-9a31-c10b07816787.xml"}, "exchange direction": "INPUT", "other": {"anies": [{"name": "referenceToUnitGroupDataSet", "value": {"shortDescription": [{"value": "MJ", "lang": "de"}], "type": "unit group data set", "refObjectId": "93a60a57-a3c8-11da-a746-0800200c9a66", "uri": "../unitgroups/93a60a57-a3c8-11da-a746-0800200c9a66.xml"}}, {"value": "0", "module": "A1-A3"}, {"value": "0", "module": "A4"}, {"value": "0", "module": "A5"}, {"value": "0", "module": "B1"}, {"value": "0", "module": "B2"}, {"value": "0", "module": "B6"}, {"value": "0", "module": "B7"}, {"value": "0", "module": "C1"}, {"value": "0", "module": "C2"}, {"value": "0", "module": "C3", "scenario": "S0"}, {"value": "0", "module": "C3", "scenario": "S1"}, {"value": "0", "module": "C3", "scenario": "S2"}, {"value": "0", "module": "C4", "scenario": "S0"}, {"value": "0", "module": "C4", "scenario": "S1"}, {"value": "0", "module": "C4", "scenario": "S2"}, {"value": "0", "module": "D", "scenario": "S0"}, {"value": "0", "module": "D", "scenario": "S1"}, {"value": "0", "module": "D", "scenario": "S2"}]}, "resolvedFlowVersion": "38.00.000", "flowProperties": [], "typeOfFlow": "Other flow", "classification": {"classHierarchy": "Quantities / Environmental quantities / EPD EN 15804 / LCI indicators", "name": "GaBiCategories"}}, {"dataSetInternalID": 9, "referenceToFlowDataSet": {"shortDescription": [{"value": "Nicht erneuerbare Sekundärbrennstoffe (NRSF)", "lang": "de"}, {"value": "Use of non renewable secondary fuels (NRSF)", "lang": "en"}], "type": "flow data set", "refObjectId": "89def144-d39a-4287-b86f-efde453ddcb2", "uri": "../flows/89def144-d39a-4287-b86f-efde453ddcb2.xml"}, "exchange direction": "INPUT", "other": {"anies": [{"name": "referenceToUnitGroupDataSet", "value": {"shortDescription": [{"value": "MJ", "lang": "de"}], "type": "unit group data set", "refObjectId": "93a60a57-a3c8-11da-a746-0800200c9a66", "uri": "../unitgroups/93a60a57-a3c8-11da-a746-0800200c9a66.xml"}}, {"value": "0", "module": "A1-A3"}, {"value": "0", "module": "A4"}, {"value": "0", "module": "A5"}, {"value": "0", "module": "B1"}, {"value": "0", "module": "B2"}, {"value": "0", "module": "B6"}, {"value": "0", "module": "B7"}, {"value": "0", "module": "C1"}, {"value": "0", "module": "C2"}, {"value": "0", "module": "C3", "scenario": "S0"}, {"value": "0", "module": "C3", "scenario": "S1"}, {"value": "0", "module": "C3", "scenario": "S2"}, {"value": "0", "module": "C4", "scenario": "S0"}, {"value": "0", "module": "C4", "scenario": "S1"}, {"value": "0", "module": "C4", "scenario": "S2"}, {"value": "0", "module": "D", "scenario": "S0"}, {"value": "0", "module": "D", "scenario": "S1"}, {"value": "0", "module": "D", "scenario": "S2"}]}, "resolvedFlowVersion": "38.00.000", "flowProperties": [], "typeOfFlow": "Other flow", "classification": {"classHierarchy": "Quantities / Environmental quantities / EPD EN 15804 / LCI indicators", "name": "GaBiCategories"}}, {"dataSetInternalID": 10, "referenceToFlowDataSet": {"shortDescription": [{"value": "Einsatz von Süßwasserressourcen (FW)", "lang": "de"}, {"value": "Use of net fresh water (FW)", "lang": "en"}], "type": "flow data set", "refObjectId": "3cf952c8-f3a4-461d-8c96-96456ca62246", "uri": "../flows/3cf952c8-f3a4-461d-8c96-96456ca62246.xml"}, "exchange direction": "INPUT", "other": {"anies": [{"name": "referenceToUnitGroupDataSet", "value": {"shortDescription": [{"value": "m^3", "lang": "de"}], "type": "unit group data set", "refObjectId": "cd950537-0a98-4044-9ba7-9f9a68d0a504", "uri": "../unitgroups/cd950537-0a98-4044-9ba7-9f9a68d0a504.xml"}}, {"value": "0.00291908339351354", "module": "A1-A3"}, {"value": "5.27098310627865E-05", "module": "A4"}, {"value": "0.000594217261276966", "module": "A5"}, {"value": "0", "module": "B1"}, {"value": "5.1960228550558E-05", "module": "B2"}, {"value": "0", "module": "B6"}, {"value": "0", "module": "B7"}, {"value": "7.2629425879555E-05", "module": "C1"}, {"value": "8.50202190240759E-06", "module": "C2"}, {"value": "0.000407367571437056", "module": "C3", "scenario": "S0"}, {"value": "0.00684824025848707", "module": "C3", "scenario": "S1"}, {"value": "8.25415245539835E-05", "module": "C3", "scenario": "S2"}, {"value": "0", "module": "C4", "scenario": "S0"}, {"value": "0", "module": "C4", "scenario": "S1"}, {"value": "0.000113558034275697", "module": "C4", "scenario": "S2"}, {"value": "-0.00022980977843666", "module": "D", "scenario": "S0"}, {"value": "-0.0062583284052784", "module": "D", "scenario": "S1"}, {"value": "-7.88369299379171E-05", "module": "D", "scenario": "S2"}]}, "resolvedFlowVersion": "38.00.000", "flowProperties": [], "typeOfFlow": "Other flow", "classification": {"classHierarchy": "Quantities / Environmental quantities / EPD EN 15804 / LCI indicators", "name": "GaBiCategories"}}, {"dataSetInternalID": 11, "referenceToFlowDataSet": {"shortDescription": [{"value": "Gefährlicher Abfall zur Deponie (HWD)", "lang": "de"}, {"value": "Hazardous waste disposed (HWD)", "lang": "en"}], "type": "flow data set", "refObjectId": "430f9e0f-59b2-46a0-8e0d-55e0e84948fc", "uri": "../flows/430f9e0f-59b2-46a0-8e0d-55e0e84948fc.xml"}, "exchange direction": "OUTPUT", "other": {"anies": [{"name": "referenceToUnitGroupDataSet", "value": {"shortDescription": [{"value": "kg", "lang": "de"}], "type": "unit group data set", "refObjectId": "ad38d542-3fe9-439d-9b95-2f5f7752acaf", "uri": "../unitgroups/ad38d542-3fe9-439d-9b95-2f5f7752acaf.xml"}}, {"value": "1.68793769550102E-07", "module": "A1-A3"}, {"value": "2.10326082774229E-11", "module": "A4"}, {"value": "4.86738639407617E-10", "module": "A5"}, {"value": "0", "module": "B1"}, {"value": "1.8660711953622E-11", "module": "B2"}, {"value": "0", "module": "B6"}, {"value": "0", "module": "B7"}, {"value": "2.47500494955331E-11", "module": "C1"}, {"value": "3.39253024784714E-12", "module": "C2"}, {"value": "2.26142797822069E-10", "module": "C3", "scenario": "S0"}, {"value": "2.20502818680773E-10", "module": "C3", "scenario": "S1"}, {"value": "2.65771032197731E-12", "module": "C3", "scenario": "S2"}, {"value": "0", "module": "C4", "scenario": "S0"}, {"value": "0", "module": "C4", "scenario": "S1"}, {"value": "1.22734356436781E-10", "module": "C4", "scenario": "S2"}, {"value": "-3.891344898904E-10", "module": "D", "scenario": "S0"}, {"value": "-1.6521220288237E-08", "module": "D", "scenario": "S1"}, {"value": "-2.08120458741442E-10", "module": "D", "scenario": "S2"}]}, "resolvedFlowVersion": "38.00.000", "flowProperties": [], "typeOfFlow": "Other flow", "classification": {"classHierarchy": "Quantities / Environmental quantities / EPD EN 15804 / LCI indicators", "name": "GaBiCategories"}}, {"dataSetInternalID": 12, "referenceToFlowDataSet": {"shortDescription": [{"value": "Entsorgter nicht gefährlicher Abfall (NHWD)", "lang": "de"}, {"value": "Non hazardous waste disposed (NHWD)", "lang": "en"}], "type": "flow data set", "refObjectId": "b29ef66b-e286-4afa-949f-62f1a7b4d7fa", "uri": "../flows/b29ef66b-e286-4afa-949f-62f1a7b4d7fa.xml"}, "exchange direction": "OUTPUT", "other": {"anies": [{"name": "referenceToUnitGroupDataSet", "value": {"shortDescription": [{"value": "kg", "lang": "de"}], "type": "unit group data set", "refObjectId": "ad38d542-3fe9-439d-9b95-2f5f7752acaf", "uri": "../unitgroups/ad38d542-3fe9-439d-9b95-2f5f7752acaf.xml"}}, {"value": "0.00811005641617289", "module": "A1-A3"}, {"value": "8.96946466470143E-05", "module": "A4"}, {"value": "0.276772599399495", "module": "A5"}, {"value": "0", "module": "B1"}, {"value": "0.00410317882710001", "module": "B2"}, {"value": "0", "module": "B6"}, {"value": "0", "module": "B7"}, {"value": "0.000118983054045623", "module": "C1"}, {"value": "1.44676208393323E-05", "module": "C2"}, {"value": "0.0017229014981047", "module": "C3", "scenario": "S0"}, {"value": "0.0125696318631692", "module": "C3", "scenario": "S1"}, {"value": "0.000151501194161889", "module": "C3", "scenario": "S2"}, {"value": "0", "module": "C4", "scenario": "S0"}, {"value": "0", "module": "C4", "scenario": "S1"}, {"value": "0.995859757410368", "module": "C4", "scenario": "S2"}, {"value": "-0.000173227798978225", "module": "D", "scenario": "S0"}, {"value": "-0.0127828976172422", "module": "D", "scenario": "S1"}, {"value": "-0.000161042867876318", "module": "D", "scenario": "S2"}]}, "resolvedFlowVersion": "38.00.000", "flowProperties": [], "typeOfFlow": "Other flow", "classification": {"classHierarchy": "Quantities / Environmental quantities / EPD EN 15804 / LCI indicators", "name": "GaBiCategories"}}, {"dataSetInternalID": 13, "referenceToFlowDataSet": {"shortDescription": [{"value": "Entsorgter radioaktiver Abfall (RWD)", "lang": "de"}, {"value": "Radioactive waste disposed (RWD)", "lang": "en"}], "type": "flow data set", "refObjectId": "3449546e-52ad-4b39-b809-9fb77cea8ff6", "uri": "../flows/3449546e-52ad-4b39-b809-9fb77cea8ff6.xml"}, "exchange direction": "OUTPUT", "other": {"anies": [{"name": "referenceToUnitGroupDataSet", "value": {"shortDescription": [{"value": "kg", "lang": "de"}], "type": "unit group data set", "refObjectId": "ad38d542-3fe9-439d-9b95-2f5f7752acaf", "uri": "../unitgroups/ad38d542-3fe9-439d-9b95-2f5f7752acaf.xml"}}, {"value": "0.000167197314389901", "module": "A1-A3"}, {"value": "1.00054580833887E-06", "module": "A4"}, {"value": "3.27434636702652E-05", "module": "A5"}, {"value": "0", "module": "B1"}, {"value": "2.42223832095271E-06", "module": "B2"}, {"value": "0", "module": "B6"}, {"value": "0", "module": "B7"}, {"value": "9.88771452331734E-07", "module": "C1"}, {"value": "1.61386637091032E-07", "module": "C2"}, {"value": "0.00014777214566886", "module": "C3", "scenario": "S0"}, {"value": "2.10332296712595E-05", "module": "C3", "scenario": "S1"}, {"value": "2.53512548892873E-07", "module": "C3", "scenario": "S2"}, {"value": "0", "module": "C4", "scenario": "S0"}, {"value": "0", "module": "C4", "scenario": "S1"}, {"value": "7.00700239681044E-06", "module": "C4", "scenario": "S2"}, {"value": "2.07770085783814E-05", "module": "D", "scenario": "S0"}, {"value": "-0.00180282759913154", "module": "D", "scenario": "S1"}, {"value": "-2.27104065061082E-05", "module": "D", "scenario": "S2"}]}, "resolvedFlowVersion": "38.00.000", "flowProperties": [], "typeOfFlow": "Other flow", "classification": {"classHierarchy": "Quantities / Environmental quantities / EPD EN 15804 / LCI indicators", "name": "GaBiCategories"}}, {"dataSetInternalID": 14, "referenceToFlowDataSet": {"shortDescription": [{"value": "Komponenten für die Wiederverwendung (CRU)", "lang": "de"}, {"value": "Components for re-use (CRU)", "lang": "en"}], "type": "flow data set", "refObjectId": "a2b32f97-3fc7-4af2-b209-525bc6426f33", "uri": "../flows/a2b32f97-3fc7-4af2-b209-525bc6426f33.xml"}, "exchange direction": "OUTPUT", "other": {"anies": [{"name": "referenceToUnitGroupDataSet", "value": {"shortDescription": [{"value": "kg", "lang": "de"}], "type": "unit group data set", "refObjectId": "ad38d542-3fe9-439d-9b95-2f5f7752acaf", "uri": "../unitgroups/ad38d542-3fe9-439d-9b95-2f5f7752acaf.xml"}}, {"value": "0", "module": "A1-A3"}, {"value": "0", "module": "A4"}, {"value": "0", "module": "A5"}, {"value": "0", "module": "B1"}, {"value": "0", "module": "B2"}, {"value": "0", "module": "B6"}, {"value": "0", "module": "B7"}, {"value": "0", "module": "C1"}, {"value": "0", "module": "C2"}, {"value": "0", "module": "C3", "scenario": "S0"}, {"value": "0", "module": "C3", "scenario": "S1"}, {"value": "0", "module": "C3", "scenario": "S2"}, {"value": "0", "module": "C4", "scenario": "S0"}, {"value": "0", "module": "C4", "scenario": "S1"}, {"value": "0", "module": "C4", "scenario": "S2"}, {"value": "0", "module": "D", "scenario": "S0"}, {"value": "0", "module": "D", "scenario": "S1"}, {"value": "0", "module": "D", "scenario": "S2"}]}, "resolvedFlowVersion": "38.00.000", "flowProperties": [], "typeOfFlow": "Other flow", "classification": {"classHierarchy": "Quantities / Environmental quantities / EPD EN 15804 / LCI indicators", "name": "GaBiCategories"}}, {"dataSetInternalID": 15, "referenceToFlowDataSet": {"shortDescription": [{"value": "Stoffe zum Recycling (MFR)", "lang": "de"}, {"value": "Materials for recycling (MFR)", "lang": "en"}], "type": "flow data set", "refObjectId": "d7fe48a5-4103-49c8-9aae-b0b5dfdbd6ae", "uri": "../flows/d7fe48a5-4103-49c8-9aae-b0b5dfdbd6ae.xml"}, "exchange direction": "OUTPUT", "other": {"anies": [{"name": "referenceToUnitGroupDataSet", "value": {"shortDescription": [{"value": "kg", "lang": "de"}], "type": "unit group data set", "refObjectId": "ad38d542-3fe9-439d-9b95-2f5f7752acaf", "uri": "../unitgroups/ad38d542-3fe9-439d-9b95-2f5f7752acaf.xml"}}, {"value": "0.037909747968", "module": "A1-A3"}, {"value": "0", "module": "A4"}, {"value": "0", "module": "A5"}, {"value": "0", "module": "B1"}, {"value": "0", "module": "B2"}, {"value": "0", "module": "B6"}, {"value": "0", "module": "B7"}, {"value": "0", "module": "C1"}, {"value": "0", "module": "C2"}, {"value": "0.9603", "module": "C3", "scenario": "S0"}, {"value": "0", "module": "C3", "scenario": "S1"}, {"value": "0", "module": "C3", "scenario": "S2"}, {"value": "0", "module": "C4", "scenario": "S0"}, {"value": "0", "module": "C4", "scenario": "S1"}, {"value": "0", "module": "C4", "scenario": "S2"}, {"value": "0", "module": "D", "scenario": "S0"}, {"value": "0", "module": "D", "scenario": "S1"}, {"value": "0", "module": "D", "scenario": "S2"}]}, "resolvedFlowVersion": "38.00.000", "flowProperties": [], "typeOfFlow": "Other flow", "classification": {"classHierarchy": "Quantities / Environmental quantities / EPD EN 15804 / LCI indicators", "name": "GaBiCategories"}}, {"dataSetInternalID": 16, "referenceToFlowDataSet": {"shortDescription": [{"value": "Stoffe für die Energierückgewinnung (MER)", "lang": "de"}, {"value": "Materials for energy recovery (MER)", "lang": "en"}], "type": "flow data set", "refObjectId": "59a9181c-3aaf-46ee-8b13-2b3723b6e447", "uri": "../flows/59a9181c-3aaf-46ee-8b13-2b3723b6e447.xml"}, "exchange direction": "OUTPUT", "other": {"anies": [{"name": "referenceToUnitGroupDataSet", "value": {"shortDescription": [{"value": "kg", "lang": "de"}], "type": "unit group data set", "refObjectId": "ad38d542-3fe9-439d-9b95-2f5f7752acaf", "uri": "../unitgroups/ad38d542-3fe9-439d-9b95-2f5f7752acaf.xml"}}, {"value": "0", "module": "A1-A3"}, {"value": "0", "module": "A4"}, {"value": "0", "module": "A5"}, {"value": "0", "module": "B1"}, {"value": "0", "module": "B2"}, {"value": "0", "module": "B6"}, {"value": "0", "module": "B7"}, {"value": "0", "module": "C1"}, {"value": "0", "module": "C2"}, {"value": "0", "module": "C3", "scenario": "S0"}, {"value": "0", "module": "C3", "scenario": "S1"}, {"value": "0", "module": "C3", "scenario": "S2"}, {"value": "0", "module": "C4", "scenario": "S0"}, {"value": "0", "module": "C4", "scenario": "S1"}, {"value": "0", "module": "C4", "scenario": "S2"}, {"value": "0", "module": "D", "scenario": "S0"}, {"value": "0", "module": "D", "scenario": "S1"}, {"value": "0", "module": "D", "scenario": "S2"}]}, "resolvedFlowVersion": "38.00.000", "flowProperties": [], "typeOfFlow": "Other flow", "classification": {"classHierarchy": "Quantities / Environmental quantities / EPD EN 15804 / LCI indicators", "name": "GaBiCategories"}}, {"dataSetInternalID": 17, "referenceToFlowDataSet": {"shortDescription": [{"value": "Exportierte elektrische Energie (EEE)", "lang": "de"}, {"value": "Exported electrical energy (EEE)", "lang": "en"}], "type": "flow data set", "refObjectId": "4da0c987-2b76-40d6-9e9e-82a017aaaf29", "uri": "../flows/4da0c987-2b76-40d6-9e9e-82a017aaaf29.xml"}, "exchange direction": "OUTPUT", "other": {"anies": [{"name": "referenceToUnitGroupDataSet", "value": {"shortDescription": [{"value": "MJ", "lang": "de"}], "type": "unit group data set", "refObjectId": "93a60a57-a3c8-11da-a746-0800200c9a66", "uri": "../unitgroups/93a60a57-a3c8-11da-a746-0800200c9a66.xml"}}, {"value": "0.0744177110608655", "module": "A1-A3"}, {"value": "0", "module": "A4"}, {"value": "0.00372678155059283", "module": "A5"}, {"value": "0", "module": "B1"}, {"value": "0", "module": "B2"}, {"value": "0", "module": "B6"}, {"value": "0", "module": "B7"}, {"value": "0", "module": "C1"}, {"value": "0", "module": "C2"}, {"value": "0.146316965965681", "module": "C3", "scenario": "S0"}, {"value": "6.76264990641379", "module": "C3", "scenario": "S1"}, {"value": "0.0815099079808815", "module": "C3", "scenario": "S2"}, {"value": "0", "module": "C4", "scenario": "S0"}, {"value": "0", "module": "C4", "scenario": "S1"}, {"value": "0", "module": "C4", "scenario": "S2"}, {"value": "0", "module": "D", "scenario": "S0"}, {"value": "0", "module": "D", "scenario": "S1"}, {"value": "0", "module": "D", "scenario": "S2"}]}, "resolvedFlowVersion": "38.00.000", "flowProperties": [], "typeOfFlow": "Other flow", "classification": {"classHierarchy": "Quantities / Environmental quantities / EPD EN 15804 / LCI indicators", "name": "GaBiCategories"}}, {"dataSetInternalID": 18, "referenceToFlowDataSet": {"shortDescription": [{"value": "Exportierte thermische Energie (EET)", "lang": "de"}, {"value": "Exported thermal energy (EET)", "lang": "en"}], "type": "flow data set", "refObjectId": "98daf38a-7a79-46d3-9a37-2b7bd0955810", "uri": "../flows/98daf38a-7a79-46d3-9a37-2b7bd0955810.xml"}, "exchange direction": "OUTPUT", "other": {"anies": [{"name": "referenceToUnitGroupDataSet", "value": {"shortDescription": [{"value": "MJ", "lang": "de"}], "type": "unit group data set", "refObjectId": "93a60a57-a3c8-11da-a746-0800200c9a66", "uri": "../unitgroups/93a60a57-a3c8-11da-a746-0800200c9a66.xml"}}, {"value": "0.152025657858295", "module": "A1-A3"}, {"value": "0", "module": "A4"}, {"value": "0.00668122865849056", "module": "A5"}, {"value": "0", "module": "B1"}, {"value": "0", "module": "B2"}, {"value": "0", "module": "B6"}, {"value": "0", "module": "B7"}, {"value": "0", "module": "C1"}, {"value": "0", "module": "C2"}, {"value": "0.260171667613849", "module": "C3", "scenario": "S0"}, {"value": "12.0249206373853", "module": "C3", "scenario": "S1"}, {"value": "0.144935814835112", "module": "C3", "scenario": "S2"}, {"value": "0", "module": "C4", "scenario": "S0"}, {"value": "0", "module": "C4", "scenario": "S1"}, {"value": "0", "module": "C4", "scenario": "S2"}, {"value": "0", "module": "D", "scenario": "S0"}, {"value": "0", "module": "D", "scenario": "S1"}, {"value": "0", "module": "D", "scenario": "S2"}]}, "resolvedFlowVersion": "38.00.000", "flowProperties": [], "typeOfFlow": "Other flow", "classification": {"classHierarchy": "Quantities / Environmental quantities / EPD EN 15804 / LCI indicators", "name": "GaBiCategories"}}]}, "LCIAResults": {"LCIAResult": [{"referenceToLCIAMethodDataSet": {"shortDescription": [{"value": "Globales Erwärmungspotenzial total (GWP-total)", "lang": "de"}, {"value": "Global Warming Potential total (GWP-total)", "lang": "en"}], "type": "LCIA method data set", "refObjectId": "6a37f984-a4b3-458a-a20a-64418c145fa2", "uri": "../lciamethods/6a37f984-a4b3-458a-a20a-64418c145fa2.xml"}, "other": {"anies": [{"name": "referenceToUnitGroupDataSet", "value": {"shortDescription": [{"value": "kg CO_(2)-Äq.", "lang": "de"}], "type": "unit group data set", "refObjectId": "1ebf3012-d0db-4de2-aefd-ef30cedb0be1", "uri": "../unitgroups/1ebf3012-d0db-4de2-aefd-ef30cedb0be1.xml"}}, {"value": "0.577563081285288", "module": "A1-A3"}, {"value": "0.0424523349477735", "module": "A4"}, {"value": "0.352715355435748", "module": "A5"}, {"value": "0", "module": "B1"}, {"value": "0.0172646597037255", "module": "B2"}, {"value": "0", "module": "B6"}, {"value": "0", "module": "B7"}, {"value": "0.0598424564260526", "module": "C1"}, {"value": "0.0068475021501093", "module": "C2"}, {"value": "0.223169031174806", "module": "C3", "scenario": "S0"}, {"value": "3.16834009477603", "module": "C3", "scenario": "S1"}, {"value": "0.0381878572972412", "module": "C3", "scenario": "S2"}, {"value": "0", "module": "C4", "scenario": "S0"}, {"value": "0", "module": "C4", "scenario": "S1"}, {"value": "0.0294187429301967", "module": "C4", "scenario": "S2"}, {"value": "0.0297948271320934", "module": "D", "scenario": "S0"}, {"value": "-1.38475440866563", "module": "D", "scenario": "S1"}, {"value": "-0.0174476460381546", "module": "D", "scenario": "S2"}]}}, {"referenceToLCIAMethodDataSet": {"shortDescription": [{"value": "Globales Erwärmungspotenzial fossil (GWP-fossil)", "lang": "de"}, {"value": "Global Warming Potential fossil fuels (GWP-fossil)", "lang": "en"}], "type": "LCIA method data set", "refObjectId": "5f635281-343e-44fb-83df-1971b155e6b6", "uri": "../lciamethods/5f635281-343e-44fb-83df-1971b155e6b6.xml"}, "other": {"anies": [{"name": "referenceToUnitGroupDataSet", "value": {"shortDescription": [{"value": "kg CO_(2)-Äq.", "lang": "de"}], "type": "unit group data set", "refObjectId": "1ebf3012-d0db-4de2-aefd-ef30cedb0be1", "uri": "../unitgroups/1ebf3012-d0db-4de2-aefd-ef30cedb0be1.xml"}}, {"value": "0.565814028413231", "module": "A1-A3"}, {"value": "0.0416520416165218", "module": "A4"}, {"value": "0.350938429541316", "module": "A5"}, {"value": "0", "module": "B1"}, {"value": "0.0145605715531627", "module": "B2"}, {"value": "0", "module": "B6"}, {"value": "0", "module": "B7"}, {"value": "0.0603160063161335", "module": "C1"}, {"value": "0.00671841595701283", "module": "C2"}, {"value": "0.222645612965132", "module": "C3", "scenario": "S0"}, {"value": "3.16825377435623", "module": "C3", "scenario": "S1"}, {"value": "0.0381868168811954", "module": "C3", "scenario": "S2"}, {"value": "0", "module": "C4", "scenario": "S0"}, {"value": "0", "module": "C4", "scenario": "S1"}, {"value": "0.0293914343736044", "module": "C4", "scenario": "S2"}, {"value": "0.0300544562921119", "module": "D", "scenario": "S0"}, {"value": "-1.3786763277364", "module": "D", "scenario": "S1"}, {"value": "-0.0173710747394064", "module": "D", "scenario": "S2"}]}}, {"referenceToLCIAMethodDataSet": {"shortDescription": [{"value": "Globales Erwärmungspotenzial biogen (GWP-biogenic)", "lang": "de"}, {"value": "Global Warming Potential biogenic (GWP-biogenic)", "lang": "en"}], "type": "LCIA method data set", "refObjectId": "2356e1ab-0185-4db5-86e5-16de51c7485c", "uri": "../lciamethods/2356e1ab-0185-4db5-86e5-16de51c7485c.xml"}, "other": {"anies": [{"name": "referenceToUnitGroupDataSet", "value": {"shortDescription": [{"value": "kg CO_(2)-Äq.", "lang": "de"}], "type": "unit group data set", "refObjectId": "1ebf3012-d0db-4de2-aefd-ef30cedb0be1", "uri": "../unitgroups/1ebf3012-d0db-4de2-aefd-ef30cedb0be1.xml"}}, {"value": "0.0107239491193031", "module": "A1-A3"}, {"value": "9.95462047846964E-05", "module": "A4"}, {"value": "0", "module": "A5"}, {"value": "0", "module": "B1"}, {"value": "0.00269976513943014", "module": "B2"}, {"value": "0", "module": "B6"}, {"value": "0", "module": "B7"}, {"value": "0", "module": "C1"}, {"value": "1.60566633646184E-05", "module": "C2"}, {"value": "0.000507121175955399", "module": "C3", "scenario": "S0"}, {"value": "7.99773656673499E-05", "module": "C3", "scenario": "S1"}, {"value": "9.63963506364026E-07", "module": "C3", "scenario": "S2"}, {"value": "0", "module": "C4", "scenario": "S0"}, {"value": "0", "module": "C4", "scenario": "S1"}, {"value": "0", "module": "C4", "scenario": "S2"}, {"value": "-0.000257404306298843", "module": "D", "scenario": "S0"}, {"value": "-0.00595296000265638", "module": "D", "scenario": "S1"}, {"value": "-7.49949453795126E-05", "module": "D", "scenario": "S2"}]}}, {"referenceToLCIAMethodDataSet": {"shortDescription": [{"value": "Globales Erwärmungspotenzial luluc (GWP-luluc)", "lang": "de"}, {"value": "Global Warming Potential luluc (GWP-luluc)", "lang": "en"}], "type": "LCIA method data set", "refObjectId": "4331bbdb-978a-490d-8707-eeb047f01a55", "uri": "../lciamethods/4331bbdb-978a-490d-8707-eeb047f01a55.xml"}, "other": {"anies": [{"name": "referenceToUnitGroupDataSet", "value": {"shortDescription": [{"value": "kg CO_(2)-Äq.", "lang": "de"}], "type": "unit group data set", "refObjectId": "1ebf3012-d0db-4de2-aefd-ef30cedb0be1", "uri": "../unitgroups/1ebf3012-d0db-4de2-aefd-ef30cedb0be1.xml"}}, {"value": "0.00102510375275322", "module": "A1-A3"}, {"value": "0.000700747126467076", "module": "A4"}, {"value": "0.00511182211400239", "module": "A5"}, {"value": "0", "module": "B1"}, {"value": "4.32301113266092E-06", "module": "B2"}, {"value": "0", "module": "B6"}, {"value": "0", "module": "B7"}, {"value": "0.000984849592446106", "module": "C1"}, {"value": "0.000113029529731859", "module": "C2"}, {"value": "1.6297033718131E-05", "module": "C3", "scenario": "S0"}, {"value": "6.34305413185642E-06", "module": "C3", "scenario": "S1"}, {"value": "7.64525394276312E-08", "module": "C3", "scenario": "S2"}, {"value": "0", "module": "C4", "scenario": "S0"}, {"value": "0", "module": "C4", "scenario": "S1"}, {"value": "0.000108276659415274", "module": "C4", "scenario": "S2"}, {"value": "-2.22485371971564E-06", "module": "D", "scenario": "S0"}, {"value": "-0.000125120926567798", "module": "D", "scenario": "S1"}, {"value": "-1.5763533686269E-06", "module": "D", "scenario": "S2"}]}}, {"referenceToLCIAMethodDataSet": {"shortDescription": [{"value": "Abbau Potential der stratosphärischen Ozonschicht (ODP)", "lang": "de"}, {"value": "Depletion potential of the stratospheric ozone layer (ODP)", "lang": "en"}], "type": "LCIA method data set", "refObjectId": "b5c629d6-def3-11e6-bf01-fe55135034f3", "uri": "../lciamethods/b5c629d6-def3-11e6-bf01-fe55135034f3.xml"}, "other": {"anies": [{"name": "referenceToUnitGroupDataSet", "value": {"shortDescription": [{"value": "kg CFC11-Äq.", "lang": "de"}], "type": "unit group data set", "refObjectId": "d9e957c9-7309-4474-bf3a-7777df6c4e5b", "uri": "../unitgroups/d9e957c9-7309-4474-bf3a-7777df6c4e5b.xml"}}, {"value": "2.20096280035592E-11", "module": "A1-A3"}, {"value": "6.14260481145216E-15", "module": "A4"}, {"value": "3.02985074531362E-13", "module": "A5"}, {"value": "0", "module": "B1"}, {"value": "1.09427084086623E-14", "module": "B2"}, {"value": "0", "module": "B6"}, {"value": "0", "module": "B7"}, {"value": "5.90427040794708E-15", "module": "C1"}, {"value": "9.90793550117704E-16", "module": "C2"}, {"value": "1.87414978115678E-14", "module": "C3", "scenario": "S0"}, {"value": "1.68182366099939E-13", "module": "C3", "scenario": "S1"}, {"value": "2.0270943157669E-15", "module": "C3", "scenario": "S2"}, {"value": "0", "module": "C4", "scenario": "S0"}, {"value": "0", "module": "C4", "scenario": "S1"}, {"value": "9.69674276482853E-14", "module": "C4", "scenario": "S2"}, {"value": "-3.57414431758291E-13", "module": "D", "scenario": "S0"}, {"value": "-1.22407799828219E-11", "module": "D", "scenario": "S1"}, {"value": "-1.54198384546968E-13", "module": "D", "scenario": "S2"}]}}, {"referenceToLCIAMethodDataSet": {"shortDescription": [{"value": "Versauerungspotenzial von Boden und Wasser (AP)", "lang": "de"}, {"value": "Acidification potential of land and water (AP)", "lang": "en"}], "type": "LCIA method data set", "refObjectId": "b5c611c6-def3-11e6-bf01-fe55135034f3", "uri": "../lciamethods/b5c611c6-def3-11e6-bf01-fe55135034f3.xml"}, "other": {"anies": [{"name": "referenceToUnitGroupDataSet", "value": {"shortDescription": [{"value": "mol H^(+)-Äq.", "lang": "de"}], "type": "unit group data set", "refObjectId": "42e089ac-92bf-4bf2-8ca1-5fc40d18f2ed", "uri": "../unitgroups/42e089ac-92bf-4bf2-8ca1-5fc40d18f2ed.xml"}}, {"value": "0.000994350746879762", "module": "A1-A3"}, {"value": "6.68130122647962E-05", "module": "A4"}, {"value": "0.00111409698268405", "module": "A5"}, {"value": "0", "module": "B1"}, {"value": "5.76180946957533E-05", "module": "B2"}, {"value": "0", "module": "B6"}, {"value": "0", "module": "B7"}, {"value": "0.000292007654878373", "module": "C1"}, {"value": "1.07768452713215E-05", "module": "C2"}, {"value": "0.000193220002380833", "module": "C3", "scenario": "S0"}, {"value": "0.000315761930881014", "module": "C3", "scenario": "S1"}, {"value": "3.80586401575615E-06", "module": "C3", "scenario": "S2"}, {"value": "0", "module": "C4", "scenario": "S0"}, {"value": "0", "module": "C4", "scenario": "S1"}, {"value": "0.000175949093858061", "module": "C4", "scenario": "S2"}, {"value": "1.14891951435093E-05", "module": "D", "scenario": "S0"}, {"value": "-0.00144117519855634", "module": "D", "scenario": "S1"}, {"value": "-1.81564241291395E-05", "module": "D", "scenario": "S2"}]}}, {"referenceToLCIAMethodDataSet": {"shortDescription": [{"value": "Eutrophierungspotenzial Süßwasser (EP-freshwater)", "lang": "de"}, {"value": "Eutrophication potential aquatic freshwater (EP-freshwater)", "lang": "en"}], "type": "LCIA method data set", "refObjectId": "b53ec18f-7377-4ad3-86eb-cc3f4f276b2b", "uri": "../lciamethods/b53ec18f-7377-4ad3-86eb-cc3f4f276b2b.xml"}, "other": {"anies": [{"name": "referenceToUnitGroupDataSet", "value": {"shortDescription": [{"value": "kg P-Äq.", "lang": "de"}], "type": "unit group data set", "refObjectId": "0429039d-a61d-4590-ba67-aa4a20a810a1", "uri": "../unitgroups/0429039d-a61d-4590-ba67-aa4a20a810a1.xml"}}, {"value": "4.63641055087224E-06", "module": "A1-A3"}, {"value": "1.78054176078438E-07", "module": "A4"}, {"value": "1.37597208035932E-06", "module": "A5"}, {"value": "0", "module": "B1"}, {"value": "2.42351296099809E-06", "module": "B2"}, {"value": "0", "module": "B6"}, {"value": "0", "module": "B7"}, {"value": "2.50163780627195E-07", "module": "C1"}, {"value": "2.87198891423283E-08", "module": "C2"}, {"value": "5.92662330527092E-07", "module": "C3", "scenario": "S0"}, {"value": "3.61851549129375E-08", "module": "C3", "scenario": "S1"}, {"value": "4.36138006261448E-10", "module": "C3", "scenario": "S2"}, {"value": "0", "module": "C4", "scenario": "S0"}, {"value": "0", "module": "C4", "scenario": "S1"}, {"value": "1.68642876493414E-05", "module": "C4", "scenario": "S2"}, {"value": "-7.25528501384189E-08", "module": "D", "scenario": "S0"}, {"value": "-2.29373688671035E-06", "module": "D", "scenario": "S1"}, {"value": "-2.88946380535272E-08", "module": "D", "scenario": "S2"}]}}, {"referenceToLCIAMethodDataSet": {"shortDescription": [{"value": "Eutrophierungspotenzial Salzwasser (EP-marine)", "lang": "de"}, {"value": "Eutrophication potential aquatic marine (EP-marine)", "lang": "en"}], "type": "LCIA method data set", "refObjectId": "b5c619fa-def3-11e6-bf01-fe55135034f3", "uri": "../lciamethods/b5c619fa-def3-11e6-bf01-fe55135034f3.xml"}, "other": {"anies": [{"name": "referenceToUnitGroupDataSet", "value": {"shortDescription": [{"value": "kg N-Äq.", "lang": "de"}], "type": "unit group data set", "refObjectId": "d05bb823-ecdf-4686-8c40-bf1d9257859f", "uri": "../unitgroups/d05bb823-ecdf-4686-8c40-bf1d9257859f.xml"}}, {"value": "0.000308392086271448", "module": "A1-A3"}, {"value": "2.489411035616E-05", "module": "A4"}, {"value": "0.000484700714410379", "module": "A5"}, {"value": "0", "module": "B1"}, {"value": "3.51918126189348E-05", "module": "B2"}, {"value": "0", "module": "B6"}, {"value": "0", "module": "B7"}, {"value": "0.000137315961271975", "module": "C1"}, {"value": "4.01538512306974E-06", "module": "C2"}, {"value": "5.63249376958125E-05", "module": "C3", "scenario": "S0"}, {"value": "6.79117957535739E-05", "module": "C3", "scenario": "S1"}, {"value": "8.18537747672003E-07", "module": "C3", "scenario": "S2"}, {"value": "0", "module": "C4", "scenario": "S0"}, {"value": "0", "module": "C4", "scenario": "S1"}, {"value": "3.78634473115985E-05", "module": "C4", "scenario": "S2"}, {"value": "1.3274158536422E-06", "module": "D", "scenario": "S0"}, {"value": "-0.000440741718837427", "module": "D", "scenario": "S1"}, {"value": "-5.55287613337756E-06", "module": "D", "scenario": "S2"}]}}, {"referenceToLCIAMethodDataSet": {"shortDescription": [{"value": "Eutrophierungspotenzial Land (EP-terrestrial)", "lang": "de"}, {"value": "Eutrophication potential terrestrial (EP-terrestrial)", "lang": "en"}], "type": "LCIA method data set", "refObjectId": "b5c614d2-def3-11e6-bf01-fe55135034f3", "uri": "../lciamethods/b5c614d2-def3-11e6-bf01-fe55135034f3.xml"}, "other": {"anies": [{"name": "referenceToUnitGroupDataSet", "value": {"shortDescription": [{"value": "mol N-Äq.", "lang": "de"}], "type": "unit group data set", "refObjectId": "71b4d617-0ec9-4d3f-b65e-e438940c2401", "uri": "../unitgroups/71b4d617-0ec9-4d3f-b65e-e438940c2401.xml"}}, {"value": "0.00321474576929649", "module": "A1-A3"}, {"value": "0.000292333488761109", "module": "A4"}, {"value": "0.00542343931233877", "module": "A5"}, {"value": "0", "module": "B1"}, {"value": "0.000284631949551033", "module": "B2"}, {"value": "0", "module": "B6"}, {"value": "0", "module": "B7"}, {"value": "0.00152285193798512", "module": "C1"}, {"value": "4.71529821693738E-05", "module": "C2"}, {"value": "0.000606106133710757", "module": "C3", "scenario": "S0"}, {"value": "0.00149943391908346", "module": "C3", "scenario": "S1"}, {"value": "1.80726079952759E-05", "module": "C3", "scenario": "S2"}, {"value": "0", "module": "C4", "scenario": "S0"}, {"value": "0", "module": "C4", "scenario": "S1"}, {"value": "0.000415836896005063", "module": "C4", "scenario": "S2"}, {"value": "2.54537184379238E-05", "module": "D", "scenario": "S0"}, {"value": "-0.00473026330803664", "module": "D", "scenario": "S1"}, {"value": "-5.95965868029724E-05", "module": "D", "scenario": "S2"}]}}, {"referenceToLCIAMethodDataSet": {"shortDescription": [{"value": "Bildungspotential für troposphärisches Ozon (POCP)", "lang": "de"}, {"value": "Formation potential of tropospheric ozone photochemical oxidants (POCP)", "lang": "en"}], "type": "LCIA method data set", "refObjectId": "b5c610fe-def3-11e6-bf01-fe55135034f3", "uri": "../lciamethods/b5c610fe-def3-11e6-bf01-fe55135034f3.xml"}, "other": {"anies": [{"name": "referenceToUnitGroupDataSet", "value": {"shortDescription": [{"value": "kg NMVOC-Äq.", "lang": "de"}], "type": "unit group data set", "refObjectId": "d27c25f8-fbc1-44c6-b47b-4adbae4199c6", "uri": "../unitgroups/d27c25f8-fbc1-44c6-b47b-4adbae4199c6.xml"}}, {"value": "0.000977383180626462", "module": "A1-A3"}, {"value": "6.47608110753864E-05", "module": "A4"}, {"value": "0.00137055187796578", "module": "A5"}, {"value": "0", "module": "B1"}, {"value": "7.51596270117065E-05", "module": "B2"}, {"value": "0", "module": "B6"}, {"value": "0", "module": "B7"}, {"value": "0.000390270224839584", "module": "C1"}, {"value": "1.04458280946638E-05", "module": "C2"}, {"value": "0.000155225562254523", "module": "C3", "scenario": "S0"}, {"value": "0.000202042786989542", "module": "C3", "scenario": "S1"}, {"value": "2.43521240987197E-06", "module": "C3", "scenario": "S2"}, {"value": "0", "module": "C4", "scenario": "S0"}, {"value": "0", "module": "C4", "scenario": "S1"}, {"value": "0.000121234249503819", "module": "C4", "scenario": "S2"}, {"value": "-1.35930800259975E-05", "module": "D", "scenario": "S0"}, {"value": "-0.00124804579415009", "module": "D", "scenario": "S1"}, {"value": "-1.57242666713975E-05", "module": "D", "scenario": "S2"}]}}, {"referenceToLCIAMethodDataSet": {"shortDescription": [{"value": "Potenzial für den abiotischen Abbau nicht fossiler Ressourcen (ADPE)", "lang": "de"}, {"value": "Abiotic depletion potential for non fossil resources (ADPE)", "lang": "en"}], "type": "LCIA method data set", "refObjectId": "b2ad6494-c78d-11e6-9d9d-cec0c932ce01", "uri": "../lciamethods/b2ad6494-c78d-11e6-9d9d-cec0c932ce01.xml"}, "other": {"anies": [{"name": "referenceToUnitGroupDataSet", "value": {"shortDescription": [{"value": "kg Sb-Äq.", "lang": "de"}], "type": "unit group data set", "refObjectId": "54ccd2d9-a32a-4fc2-923d-f2c8c93e89d4", "uri": "../unitgroups/54ccd2d9-a32a-4fc2-923d-f2c8c93e89d4.xml"}}, {"value": "1.71028231283684E-07", "module": "A1-A3"}, {"value": "3.63214493258492E-09", "module": "A4"}, {"value": "3.04647183044095E-08", "module": "A5"}, {"value": "0", "module": "B1"}, {"value": "8.16994824868069E-10", "module": "B2"}, {"value": "0", "module": "B6"}, {"value": "0", "module": "B7"}, {"value": "4.98897972123354E-09", "module": "C1"}, {"value": "5.85859888884351E-10", "module": "C2"}, {"value": "2.25222639689335E-09", "module": "C3", "scenario": "S0"}, {"value": "1.74581274047849E-09", "module": "C3", "scenario": "S1"}, {"value": "2.10422005866801E-11", "module": "C3", "scenario": "S2"}, {"value": "0", "module": "C4", "scenario": "S0"}, {"value": "0", "module": "C4", "scenario": "S1"}, {"value": "1.95328695956324E-09", "module": "C4", "scenario": "S2"}, {"value": "-4.20124621507823E-09", "module": "D", "scenario": "S0"}, {"value": "-1.19199454195541E-07", "module": "D", "scenario": "S1"}, {"value": "-1.50164954153944E-09", "module": "D", "scenario": "S2"}]}}, {"referenceToLCIAMethodDataSet": {"shortDescription": [{"value": "Potenzial für den abiotischen Abbau fossiler Brennstoffe (ADPF)", "lang": "de"}, {"value": "Abiotic depletion potential for fossil resources (ADPF)", "lang": "en"}], "type": "LCIA method data set", "refObjectId": "b2ad6110-c78d-11e6-9d9d-cec0c932ce01", "uri": "../lciamethods/b2ad6110-c78d-11e6-9d9d-cec0c932ce01.xml"}, "other": {"anies": [{"name": "referenceToUnitGroupDataSet", "value": {"shortDescription": [{"value": "MJ", "lang": "de"}], "type": "unit group data set", "refObjectId": "93a60a57-a3c8-11da-a746-0800200c9a66", "uri": "../unitgroups/93a60a57-a3c8-11da-a746-0800200c9a66.xml"}}, {"value": "12.6904816989781", "module": "A1-A3"}, {"value": "0.5492951387072", "module": "A4"}, {"value": "5.11610172429131", "module": "A5"}, {"value": "0", "module": "B1"}, {"value": "0.180970309527814", "module": "B2"}, {"value": "0", "module": "B6"}, {"value": "0", "module": "B7"}, {"value": "0.764999759481327", "module": "C1"}, {"value": "0.0886005362948689", "module": "C2"}, {"value": "2.20626814994324", "module": "C3", "scenario": "S0"}, {"value": "0.366139414798297", "module": "C3", "scenario": "S1"}, {"value": "0.00441306151011581", "module": "C3", "scenario": "S2"}, {"value": "0", "module": "C4", "scenario": "S0"}, {"value": "0", "module": "C4", "scenario": "S1"}, {"value": "0.496534894004655", "module": "C4", "scenario": "S2"}, {"value": "-0.70210835079371", "module": "D", "scenario": "S0"}, {"value": "-24.5762856846681", "module": "D", "scenario": "S1"}, {"value": "-0.309649294853686", "module": "D", "scenario": "S2"}]}}, {"referenceToLCIAMethodDataSet": {"shortDescription": [{"value": "Wassernutzung (WDP)", "lang": "de"}, {"value": "Water use (WDP)", "lang": "en"}], "type": "LCIA method data set", "refObjectId": "b2ad66ce-c78d-11e6-9d9d-cec0c932ce01", "uri": "../lciamethods/b2ad66ce-c78d-11e6-9d9d-cec0c932ce01.xml"}, "other": {"anies": [{"name": "referenceToUnitGroupDataSet", "value": {"shortDescription": [{"value": "m^(3) Welt-Äq. entzogen", "lang": "de"}], "type": "unit group data set", "refObjectId": "6ae2df01-888e-46c8-b17d-49fa3869b476", "uri": "../unitgroups/6ae2df01-888e-46c8-b17d-49fa3869b476.xml"}}, {"value": "0.0291492078948314", "module": "A1-A3"}, {"value": "0.000645779933697643", "module": "A4"}, {"value": "0.0113411801988925", "module": "A5"}, {"value": "0", "module": "B1"}, {"value": "0.00134723599214098", "module": "B2"}, {"value": "0", "module": "B6"}, {"value": "0", "module": "B7"}, {"value": "0.000872856840857347", "module": "C1"}, {"value": "0.000104163398548798", "module": "C2"}, {"value": "0.0168578687376764", "module": "C3", "scenario": "S0"}, {"value": "0.292470386270047", "module": "C3", "scenario": "S1"}, {"value": "0.00352513210086403", "module": "C3", "scenario": "S2"}, {"value": "0", "module": "C4", "scenario": "S0"}, {"value": "0", "module": "C4", "scenario": "S1"}, {"value": "0.0037977970429434", "module": "C4", "scenario": "S2"}, {"value": "0.00263891031688845", "module": "D", "scenario": "S0"}, {"value": "-0.147669330231466", "module": "D", "scenario": "S1"}, {"value": "-0.00186020896624234", "module": "D", "scenario": "S2"}]}}, {"referenceToLCIAMethodDataSet": {"shortDescription": [{"value": "Auftreten von Krankheiten aufgrund von Feinstaubemissionen (PM)", "lang": "de"}, {"value": "Incidence of disease due to PM emissions (PM)", "lang": "en"}], "type": "LCIA method data set", "refObjectId": "b5c602c6-def3-11e6-bf01-fe55135034f3", "uri": "../lciamethods/b5c602c6-def3-11e6-bf01-fe55135034f3.xml"}, "other": {"anies": [{"name": "referenceToUnitGroupDataSet", "value": {"shortDescription": [{"value": "Krankheitsfälle", "lang": "de"}], "type": "unit group data set", "refObjectId": "3883559b-648f-4afc-8ba2-0bd24f3affa3", "uri": "../unitgroups/3883559b-648f-4afc-8ba2-0bd24f3affa3.xml"}}, {"value": "1.95570101144109E-08", "module": "A1-A3"}, {"value": "6.95892102371427E-10", "module": "A4"}, {"value": "1.69159977920174E-08", "module": "A5"}, {"value": "0", "module": "B1"}, {"value": "6.68566885631729E-10", "module": "B2"}, {"value": "0", "module": "B6"}, {"value": "0", "module": "B7"}, {"value": "3.46253417262276E-09", "module": "C1"}, {"value": "1.12246421147262E-10", "module": "C2"}, {"value": "1.75526823678483E-09", "module": "C3", "scenario": "S0"}, {"value": "1.84304605653281E-09", "module": "C3", "scenario": "S1"}, {"value": "2.22141492686231E-11", "module": "C3", "scenario": "S2"}, {"value": "0", "module": "C4", "scenario": "S0"}, {"value": "0", "module": "C4", "scenario": "S1"}, {"value": "1.82161647914657E-09", "module": "C4", "scenario": "S2"}, {"value": "1.39625512800598E-10", "module": "D", "scenario": "S0"}, {"value": "-1.18128241977718E-08", "module": "D", "scenario": "S1"}, {"value": "-1.48821303185168E-10", "module": "D", "scenario": "S2"}]}}, {"referenceToLCIAMethodDataSet": {"shortDescription": [{"value": "Wirkung durch Exposition des Menschen mit U235 (IR)", "lang": "de"}, {"value": "Human exposure efficiency relative to U235 (IR)", "lang": "en"}], "type": "LCIA method data set", "refObjectId": "b5c632be-def3-11e6-bf01-fe55135034f3", "uri": "../lciamethods/b5c632be-def3-11e6-bf01-fe55135034f3.xml"}, "other": {"anies": [{"name": "referenceToUnitGroupDataSet", "value": {"shortDescription": [{"value": "kBq U235-Äq.", "lang": "de"}], "type": "unit group data set", "refObjectId": "456b05bf-1415-44a9-9993-02452f554c09", "uri": "../unitgroups/456b05bf-1415-44a9-9993-02452f554c09.xml"}}, {"value": "0.0189948820835403", "module": "A1-A3"}, {"value": "0.000145131802193752", "module": "A4"}, {"value": "0.00492539504819369", "module": "A5"}, {"value": "0", "module": "B1"}, {"value": "0.000291326870034873", "module": "B2"}, {"value": "0", "module": "B6"}, {"value": "0", "module": "B7"}, {"value": "0.000138062953886266", "module": "C1"}, {"value": "2.340955635994E-05", "module": "C2"}, {"value": "0.0137031542330611", "module": "C3", "scenario": "S0"}, {"value": "0.00336644040031662", "module": "C3", "scenario": "S1"}, {"value": "4.05755511597142E-05", "module": "C3", "scenario": "S2"}, {"value": "0", "module": "C4", "scenario": "S0"}, {"value": "0", "module": "C4", "scenario": "S1"}, {"value": "0.000960513186560129", "module": "C4", "scenario": "S2"}, {"value": "-0.00117182820095168", "module": "D", "scenario": "S0"}, {"value": "-0.296532401751679", "module": "D", "scenario": "S1"}, {"value": "-0.00373544900822676", "module": "D", "scenario": "S2"}]}}, {"referenceToLCIAMethodDataSet": {"shortDescription": [{"value": "Toxizitätsvergleichseinheit für Ökosysteme (ETP-fw)", "lang": "de"}, {"value": "Comparative toxic unit for ecosystems (ETP-fw)", "lang": "en"}], "type": "LCIA method data set", "refObjectId": "ee1082d1-b0f7-43ca-a1f0-21e2a4a74511", "uri": "../lciamethods/ee1082d1-b0f7-43ca-a1f0-21e2a4a74511.xml"}, "other": {"anies": [{"name": "referenceToUnitGroupDataSet", "value": {"shortDescription": [{"value": "CTUe", "lang": "de"}], "type": "unit group data set", "refObjectId": "aa959ded-f1eb-4efb-9c5c-2d60be36b3e6", "uri": "../unitgroups/aa959ded-f1eb-4efb-9c5c-2d60be36b3e6.xml"}}, {"value": "9.3981617656065", "module": "A1-A3"}, {"value": "0.407784286064832", "module": "A4"}, {"value": "3.53995291972936", "module": "A5"}, {"value": "0", "module": "B1"}, {"value": "0.192639242282124", "module": "B2"}, {"value": "0", "module": "B6"}, {"value": "0", "module": "B7"}, {"value": "0.562964081373529", "module": "C1"}, {"value": "0.0657750340245105", "module": "C2"}, {"value": "0.285267504931992", "module": "C3", "scenario": "S0"}, {"value": "0.151282925236193", "module": "C3", "scenario": "S1"}, {"value": "0.00182340613305824", "module": "C3", "scenario": "S2"}, {"value": "0", "module": "C4", "scenario": "S0"}, {"value": "0", "module": "C4", "scenario": "S1"}, {"value": "1.07583117021764", "module": "C4", "scenario": "S2"}, {"value": "-0.463086839869685", "module": "D", "scenario": "S0"}, {"value": "-3.45813614297269", "module": "D", "scenario": "S1"}, {"value": "-0.0435633176259616", "module": "D", "scenario": "S2"}]}}, {"referenceToLCIAMethodDataSet": {"shortDescription": [{"value": "Toxizitätsvergleichseinheit für Menschen (krebserregend) (HTP-c)", "lang": "de"}, {"value": "Comparative toxic unit for humans (carcinogenic) (HTP-c)", "lang": "en"}], "type": "LCIA method data set", "refObjectId": "2299222a-bbd8-474f-9d4f-4dd1f18aea7c", "uri": "../lciamethods/2299222a-bbd8-474f-9d4f-4dd1f18aea7c.xml"}, "other": {"anies": [{"name": "referenceToUnitGroupDataSet", "value": {"shortDescription": [{"value": "CTUh", "lang": "de"}], "type": "unit group data set", "refObjectId": "d4c9523e-2d7e-49fd-8469-998f547d3a70", "uri": "../unitgroups/d4c9523e-2d7e-49fd-8469-998f547d3a70.xml"}}, {"value": "2.99157155677273E-10", "module": "A1-A3"}, {"value": "8.23292955555503E-12", "module": "A4"}, {"value": "7.40409193688206E-11", "module": "A5"}, {"value": "0", "module": "B1"}, {"value": "5.83848076580054E-12", "module": "B2"}, {"value": "0", "module": "B6"}, {"value": "0", "module": "B7"}, {"value": "1.12865939741671E-11", "module": "C1"}, {"value": "1.32796000273521E-12", "module": "C2"}, {"value": "1.60422821458148E-11", "module": "C3", "scenario": "S0"}, {"value": "2.06516216724111E-11", "module": "C3", "scenario": "S1"}, {"value": "2.48913045251349E-13", "module": "C3", "scenario": "S2"}, {"value": "0", "module": "C4", "scenario": "S0"}, {"value": "0", "module": "C4", "scenario": "S1"}, {"value": "1.59560746630813E-11", "module": "C4", "scenario": "S2"}, {"value": "-1.30530186210524E-11", "module": "D", "scenario": "S0"}, {"value": "-2.81063493519405E-10", "module": "D", "scenario": "S1"}, {"value": "-3.54101989035302E-12", "module": "D", "scenario": "S2"}]}}, {"referenceToLCIAMethodDataSet": {"shortDescription": [{"value": "Toxizitätsvergleichseinheit für Menschen (nicht krebserregend) (HTP-nc)", "lang": "de"}, {"value": "Comparative toxic unit for humans (noncarcinogenic) (HTP-nc)", "lang": "en"}], "type": "LCIA method data set", "refObjectId": "3af763a5-b7a1-48c9-9cee-1f223481fcef", "uri": "../lciamethods/3af763a5-b7a1-48c9-9cee-1f223481fcef.xml"}, "other": {"anies": [{"name": "referenceToUnitGroupDataSet", "value": {"shortDescription": [{"value": "CTUh", "lang": "de"}], "type": "unit group data set", "refObjectId": "d4c9523e-2d7e-49fd-8469-998f547d3a70", "uri": "../unitgroups/d4c9523e-2d7e-49fd-8469-998f547d3a70.xml"}}, {"value": "5.32780565482685E-09", "module": "A1-A3"}, {"value": "3.69580234703503E-10", "module": "A4"}, {"value": "3.08083508026234E-09", "module": "A5"}, {"value": "0", "module": "B1"}, {"value": "1.47601757370176E-10", "module": "B2"}, {"value": "0", "module": "B6"}, {"value": "0", "module": "B7"}, {"value": "5.03937447131875E-10", "module": "C1"}, {"value": "5.96127740649249E-11", "module": "C2"}, {"value": "7.59722401998037E-10", "module": "C3", "scenario": "S0"}, {"value": "1.3575894613287E-10", "module": "C3", "scenario": "S1"}, {"value": "1.636296327624E-12", "module": "C3", "scenario": "S2"}, {"value": "0", "module": "C4", "scenario": "S0"}, {"value": "0", "module": "C4", "scenario": "S1"}, {"value": "3.34060502734228E-10", "module": "C4", "scenario": "S2"}, {"value": "-4.12476688621392E-10", "module": "D", "scenario": "S0"}, {"value": "-6.60992275335012E-09", "module": "D", "scenario": "S1"}, {"value": "-8.32828063641874E-11", "module": "D", "scenario": "S2"}]}}, {"referenceToLCIAMethodDataSet": {"shortDescription": [{"value": "Bodenqualitätsindex (SQP)", "lang": "de"}, {"value": "Soil quality index (SQP)", "lang": "en"}], "type": "LCIA method data set", "refObjectId": "b2ad6890-c78d-11e6-9d9d-cec0c932ce01", "uri": "../lciamethods/b2ad6890-c78d-11e6-9d9d-cec0c932ce01.xml"}, "other": {"anies": [{"name": "referenceToUnitGroupDataSet", "value": {"shortDescription": [{"value": "SQP", "lang": "de"}], "type": "unit group data set", "refObjectId": "f130951c-e67f-4f7f-8dd4-665de3974e18", "uri": "../unitgroups/f130951c-e67f-4f7f-8dd4-665de3974e18.xml"}}, {"value": "7.03186261967804", "module": "A1-A3"}, {"value": "0.270177699999238", "module": "A4"}, {"value": "2.07448993374396", "module": "A5"}, {"value": "0", "module": "B1"}, {"value": "0.0504213223641891", "module": "B2"}, {"value": "0", "module": "B6"}, {"value": "0", "module": "B7"}, {"value": "0.378663468642567", "module": "C1"}, {"value": "0.0435792844829939", "module": "C2"}, {"value": "0.160364794914776", "module": "C3", "scenario": "S0"}, {"value": "0.118864084496734", "module": "C3", "scenario": "S1"}, {"value": "0.00143266333813492", "module": "C3", "scenario": "S2"}, {"value": "0", "module": "C4", "scenario": "S0"}, {"value": "0", "module": "C4", "scenario": "S1"}, {"value": "0.0843356277405389", "module": "C4", "scenario": "S2"}, {"value": "-0.0683274324952013", "module": "D", "scenario": "S0"}, {"value": "-4.80220731796947", "module": "D", "scenario": "S1"}, {"value": "-0.0604939875280292", "module": "D", "scenario": "S2"}]}}]}, "otherAttributes": {"{http://www.indata.network/EPD/2019}epd-version": "1.2"}, "version": "1.1", "locations": "../ILCDLocations.xml"}