{"processInformation": {"dataSetInformation": {"UUID": "9cd7c3e7-6959-4f28-aa80-ede9b40bf22f", "name": {"baseName": [{"value": "Longlife-Parkett", "lang": "de"}, {"value": "Longlife parquet", "lang": "en"}], "functionalUnitFlowProperties": [{"lang": "de"}]}, "classificationInformation": {"classification": [{"class": [{"value": "Holz", "level": 0, "classId": "3"}, {"value": "Holzböden", "level": 1, "classId": "3.3"}, {"value": "Parkett", "level": 2, "classId": "3.3.02"}], "name": "OEKOBAU.DAT"}, {"class": [{"value": "02 Bauprodukte", "level": 0}, {"value": "Produkte aus Bauholz", "level": 1}, {"value": "Vollholzprodukte", "level": 2}], "name": "IBUCategories"}]}, "generalComment": [{"value": "Es handelt sich um einen dreilagig aufgebauten Mehrschicht-Parkettboden mit einer hochverdichteten Faserplatte (HDF) als Mittellage, einer Vollholz-Deckschicht aus Eiche und einem Gegenzug. Je nach Ausführungsform besteht die Deckschicht aus einer einzelnen Lamelle (Landhausdiele / 1-Stab) oder aus aufgesägten Abschnitten (Schiffsboden / 3-Stab). Die Produkte sind mit einer wohnfertig geölten oder lackierten Oberfläche ausgestattet und lassen sich als Elemente mittels spezieller Nut-Feder-Geometrie leimfrei miteinander verbinden. Die MEISTERWERKE vermarkten Parkettprodukte unter der Bezeichnung \"MeisterParkett. longlife\" (http://www.meister.com).", "lang": "de"}, {"value": "The product consists of multi-layer parquet flooring with high-density fibreboard (HDF) as a middle layer, a real wood covering layer made of oak and real wood veneer backing. Depending on the design, the top layer consists of a single lamella (plank / 1-strip) or sawn sections (ship’s floor / 3-strip). The products feature an oiled or varnished surface ready for residential use and can be joined together as elements without glue using a special tongue-and-groove geometry. MEISTERWERKE markets the parquet products under the “MeisterParkett. longlife” brand (http://meister.com).", "lang": "en"}], "other": {"anies": [{"scenario": [{"description": [{"value": "Stoffliche Verwertung", "lang": "de"}, {"value": "Material utilisation", "lang": "en"}], "name": "S1"}, {"description": [{"value": "Szenario 2", "lang": "de"}, {"value": "Scenario 2", "lang": "en"}], "name": "S2"}]}]}}, "quantitativeReference": {"referenceToReferenceFlow": [0]}, "time": {"referenceYear": 2022, "dataSetValidUntil": 2027, "other": {"anies": [{"name": "publicationDateOfEPD", "value": 1663286400000}]}}, "geography": {"locationOfOperationSupplyOrProduction": {"location": "DE"}}, "technology": {"technologyDescriptionAndIncludedProcesses": [{"value": "Zur Herstellung von MEISTER-Longlife-Parkett werden zum Teil fertige Deckschichten, Rohfriese und kammergetrocknete Hölzer verwendet, die je nach Ausführungsform formatiert, aufgetrennt und zu fertigen Deckschichten verleimt werden. Im Anschluss werden die fertigen Deckschichten je nach Wuchsmerkmalen sortiert. Für die Mittellage wird eine fertige hochverdichtete Faserplatte (HDF) und als Gegenzug ein Fichtefurnier verwendet. Die drei Schichten werden miteinander verleimt und zusammengengepresst, und anschließend in Einzelformate aufgetrennt. Bei den Einzelformaten können teilweise Äste und Risse gespachtelt werden. Die Oberfläche wird abschließend lackiert oder geölt. Für eine leimfreie Verlegung werden die Einzeldielen mit einer speziellen Nut-Feder-Geometrie ausgestattet und verpackt. \nDeklarierte Einheit: \nDie deklarierte Einheit ist 1 m² Longlife-Parkett. Bei der Durchschnittsbildung wurden die im Betrachtungszeitraum produzierten m2 für die Gewichtung der Inputs und Outputs zugrunde gelegt.", "lang": "de"}, {"value": "For the production of MEISTER Longlife parquet, partly-finished top layers, raw friezes and kiln-dried woods are used, which, depending on the design, are formatted, ripped and glued into finished top layers. The finished top layers are then sorted according to growth characteristics. A finished high-density fibreboard (HDF) is used for the middle layer and a spruce veneer is used as a backing. The three layers are glued and pressed together, and then separated into individual formats. In the case of individual formats, knots and cracks can be partially filled. The surface is then lacquered or oiled. For glue-free installation, the individual planks are equipped and packaged with a special tongue-and-groove geometry. \nDeclared unit: \nThe declared unit is 1 m² Longlife parquet. The averaging was based on the square metre produced in the period under consideration for the weighting of inputs and outputs.", "lang": "en"}], "technologicalApplicability": [{"value": "MEISTER-Longlife-Parkett sind Holzbodenprodukte nach EN 13489 die, je nach Ausführungsform, für die private und gewerbliche Nutzung im Innenbereich geeignet sind. Die Bodenbeläge werden auf Estrichen, Fliesen oder Holzunterkonstruktionen in Verbindung mit geeigneten Verlegeunterlagen (Dämmunterlagen) schwimmend verlegt oder vollflächig auf den Estrich geklebt. In allen Fällen sind die entsprechenden MEISTERWERKE-Einbaubedingungen und Unterbodenanforderungen zu beachten (http://www.meister.com).", "lang": "de"}, {"value": "MEISTER Longlife parquet are wood flooring products in accordance with EN 13489, which are suitable for private and commercial use, depending on the respective variant. The floor coverings are laid on screeds, tiles or wooden substructures in conjunction with suitable laying underlays (insulation underlays) as a floating installation or glued to the screed over the entire surface. In all cases, the corresponding MEISTERWERKE installation conditions and subfloor requirements must be observed (http://www.meister.com).", "lang": "en"}]}}, "modellingAndValidation": {"LCIMethodAndAllocation": {"typeOfDataSet": "EPD", "referenceToLCAMethodDetails": [{"shortDescription": [{"value": "Vollholzprodukte.pdf", "lang": "de"}], "type": "source data set", "refObjectId": "2c8cad11-c877-4644-b6a1-3019b825848d"}], "other": {"anies": [{"name": "subType", "value": "average dataset"}]}}, "dataSourcesTreatmentAndRepresentativeness": {"referenceToDataSource": [{"shortDescription": [{"value": "GaBi Database (all versions)", "lang": "de"}], "type": "source data set", "refObjectId": "28d74cc0-db8b-4d7e-bc44-5f6d56ce0c4a"}, {"shortDescription": [{"value": "GaBi Database Edition 2021, CUP 2021.01", "lang": "de"}], "type": "source data set", "refObjectId": "1cece811-7501-44d4-8067-9259bd5cb835"}], "useAdviceForDataSet": [{"value": "Gültigkeitsbereich: \nDiese EPD gilt für einen Quadratmeter Longlife-Parkett in den Varianten Landhausdiele und Schiffsboden, hergestellt in 59602 Rüthen-Meiste, Deutschland.  Es wird ein Durchschnitt dieser beiden Produkte deklariert. \nSystemgrenze: \nTyp der EPD: Wiege bis Werkstor mit Optionen. \n\n\nModule A1–A3 und A5 \n\nIn den Modulen A1–A3 wird die Produktion der notwendigen Rohstoffe und Energien inklusive aller entsprechenden Vorketten sowie der Beschaffungstransporte berücksichtigt. \n\nAußerdem wird die gesamte Herstellungsphase inklusive der Behandlung von Produktionsabfällen bis zum Erreichen desEnd-of-Waste Status (EoW)betrachtet. \n\nIn Modul A5 wird die Verwertung der Verpackungsmaterialien bilanziert. \n\n\nModule B2 und B5 \n\nIn Modul B2 wird die Reinigung und das Ölen des Parketts einschließlich der dafür benötigten Hilfsstoffe sowie die Behandlung der dabei anfallenden Abfälle und Abwasser betrachtet.  \n\nIn Modul B5 wird die Renovierung des Parketts einschließlich der Behandlung der dabei anfallenden Abfälle deklariert.  \n\n\nModule C1–C4 und D\n\nFür den Rückbau (Modul C1) werden keine Aufwendungen betrachtet, da ein manueller Rückbau angenommen wird.\n\nIm Modul C2 werden die Transporte zu den Entsorgungsprozessen betrachtet. \n\nDas Modul C3 beinhaltet die notwendigen Prozesse für die Abfallbehandlung am Ende des Produktlebenswegs. Es wurden zwei Szenarien betrachtet: Thermische Verwertung (Szenario 1) und stoffliche Verwertung (Szenario 2). Die Lasten für die Abfallbehandlung werden hierin soweit abgebildet, bis das Ende der Abfalleigenschaft erreicht ist. Dabei entstehende Potenziale und vermiedene Lasten außerhalb der Systemgrenze werden Modul D zugeordnet. \nEs werden keine Stoffe deponiert, sodass in Modul C4 keine Lasten/Nutzen bilanziert werden.", "lang": "de"}, {"value": "Scope: \nThis EPD applies for one square metre of Longlife parquet in the plank and 3-strip variants, manufactured in 59602 Rüthen-Meiste, Germany.  An average of these two products is declared. \nSystem boundary: \nType of EPD: Cradle to plant gate, with options \n\n\nModules A1–A3 and A5 \n\nModules A1–A3 take into account the production of the necessary raw materials and energies, including all corresponding upstream chains as well as procurement transports. \n\nIn addition, the entire manufacturing phase, including the treatment of production waste until the end-of-waste (EoW) status is reached, is considered. \n\nModule A5 balances the recycling of packaging materials. \n\n\nModules B2 and B5 \n\nModule B2 considers the cleaning and oiling of the parquet, including the ancillary materials required for this, as well as the treatment of the waste and wastewater produced in the process.  \n\nModule B5 declares the renovation of the parquet, including the treatment of the waste generated in the process.  \n\n\nModules C1–C4 and D \n\nNo expenses are considered for dismantling (Module C1), since manual dismantling is assumed. \n\nIn Module C2, the transports to the disposal processes are considered. \n\nModule C3 contains the necessary processes for waste treatment at the end of the product life cycle. Two scenarios were considered: Thermal recycling (Scenario 1) and material recycling (Scenario 2). The loads for the waste treatment are represented in this until the end of the waste property is reached. Resulting potentials and avoided loads outside the system boundary are assigned to Module D.  \n\nNo materials are landfilled, so no loads/benefits are modelled in Module C4.", "lang": "en"}], "other": {"anies": [{"name": "referenceToOriginalEPD", "value": {"shortDescription": {"value": "Longlife-Parkett.pdf", "defaultValue": "Longlife-Parkett.pdf", "lstrings": [{"lang": "de", "value": "Longlife-Parkett.pdf"}]}, "type": "source data set", "uuid": {"uuid": "5de4f127-2c79-4c99-90c9-5d865b60ddcf"}, "refObjectId": "5de4f127-2c79-4c99-90c9-5d865b60ddcf", "resourceURLs": ["https://oekobaudat.de/OEKOBAU.DAT/resource/sources/5de4f127-2c79-4c99-90c9-5d865b60ddcf/Longlife-Parkett_15156.pdf?version=00.01.000"]}}]}}, "validation": {"review": [{"referenceToNameOfReviewerAndInstitution": [{"shortDescription": [{"value": "Institut Bauen und Umwelt e. V.", "lang": "de"}], "type": "contact data set", "refObjectId": "d111dbec-b024-4be5-86c5-752d6eb2cf95", "uri": "../contacts/d111dbec-b024-4be5-86c5-752d6eb2cf95.xml"}], "type": "Accredited third party review"}]}, "complianceDeclarations": {"compliance": [{"referenceToComplianceSystem": {"shortDescription": [{"value": "DIN EN 15804+A2", "lang": "de"}], "type": "source data set", "refObjectId": "c0016b33-8cf7-415c-ac6e-deba0d21440d", "uri": "../sources/c0016b33-8cf7-415c-ac6e-deba0d21440d.xml"}}, {"referenceToComplianceSystem": {"shortDescription": [{"value": "ISO 14025", "lang": "de"}], "type": "source data set", "refObjectId": "4f2eb655-6e44-4874-a95a-e28f5442cd4d", "uri": "../sources/4f2eb655-6e44-4874-a95a-e28f5442cd4d.xml"}}]}}, "administrativeInformation": {"commissionerAndGoal": {"referenceToCommissioner": [{"shortDescription": [{"value": "MeisterWerke Schulte GmbH", "lang": "de"}], "type": "contact data set", "refObjectId": "79282f4b-72bc-4c40-a60e-5e7ac802336a", "uri": "../contacts/79282f4b-72bc-4c40-a60e-5e7ac802336a.xml"}]}, "dataGenerator": {"referenceToPersonOrEntityGeneratingTheDataSet": [{"shortDescription": [{"value": "brands and values GmbH", "lang": "de"}], "type": "contact data set", "refObjectId": "6b539b8a-10e3-4004-8ccc-a79f169aa339", "uri": "../contacts/6b539b8a-10e3-4004-8ccc-a79f169aa339.xml"}]}, "dataEntryBy": {"timeStamp": 1663334149027, "referenceToDataSetFormat": [{"shortDescription": [{"value": "ILCD Format", "lang": "de"}], "type": "source data set", "refObjectId": "a97a0155-0234-4b87-b4ce-a45da52f2a40", "uri": "../sources/a97a0155-0234-4b87-b4ce-a45da52f2a40.xml"}, {"shortDescription": [{"value": "EPD-Datenformaterweiterungen v1.2", "lang": "de"}, {"value": "EPD Data Format Extensions v1.2", "lang": "en"}], "type": "source data set", "refObjectId": "a29449fd-aa2f-4de8-b5d7-4b06b43c6fde", "uri": "../sources/a29449fd-aa2f-4de8-b5d7-4b06b43c6fde.xml"}]}, "publicationAndOwnership": {"dataSetVersion": "00.03.000", "referenceToPrecedingDataSetVersion": [{"shortDescription": [{"value": "Meister Longlife Parkett", "lang": "de"}], "type": "process data set", "refObjectId": "e74695a5-4f4b-419c-bdff-a758d20ada72", "uri": "../processes/e74695a5-4f4b-419c-bdff-a758d20ada72.xml"}], "referenceToRegistrationAuthority": {"shortDescription": [{"value": "Institut Bauen und Umwelt e. V.", "lang": "de"}], "type": "contact data set", "refObjectId": "d111dbec-b024-4be5-86c5-752d6eb2cf95", "uri": "../contacts/d111dbec-b024-4be5-86c5-752d6eb2cf95.xml"}, "registrationNumber": "EPD-MWS-20220201-ICA1-DE", "referenceToOwnershipOfDataSet": {"shortDescription": [{"value": "MeisterWerke Schulte GmbH", "lang": "de"}], "type": "contact data set", "refObjectId": "79282f4b-72bc-4c40-a60e-5e7ac802336a", "uri": "../contacts/79282f4b-72bc-4c40-a60e-5e7ac802336a.xml"}, "copyright": true, "licenseType": "Free of charge for all users and uses", "accessRestrictions": [{"value": "None", "lang": "en"}], "other": {"anies": [{"name": "referenceToPublisher", "value": {"shortDescription": [{"value": "Institut Bauen und Umwelt e. V.", "lang": "de"}], "type": "contact data set", "refObjectId": "d111dbec-b024-4be5-86c5-752d6eb2cf95", "uri": "../contacts/d111dbec-b024-4be5-86c5-752d6eb2cf95.xml"}}]}}}, "exchanges": {"exchange": [{"dataSetInternalID": 0, "referenceToFlowDataSet": {"shortDescription": [{"value": "Longlife-Parkett (1m² Longlife-Parkett)", "lang": "de"}], "type": "flow data set", "refObjectId": "b7e2ba22-5278-89be-f5b8-bfad26a6ab2b", "uri": "../flows/b7e2ba22-5278-89be-f5b8-bfad26a6ab2b.xml"}, "meanAmount": 1.0, "referencesToDataSource": {}, "referenceFlow": true, "resolvedFlowVersion": "00.04.000", "resultingflowAmount": 1.0, "flowProperties": [{"name": [{"lang": "en", "value": "Area"}, {"lang": "de", "value": "Fläche"}], "uuid": "93a60a56-a3c8-19da-a746-0800200c9a66", "referenceFlowProperty": true, "meanValue": 1.0, "referenceUnit": "qm", "unitGroupUUID": "c20a03d7-bd90-4569-bc94-66cfd364dfc8"}], "materialProperties": [{"name": "grammage", "value": "11.0", "unit": "kg/m^2", "unitDescription": "kilograms per square meter"}, {"name": "conversion factor to 1 kg", "value": "0.09", "unit": "-", "unitDescription": "Without unit"}, {"name": "gross density", "value": "500.0", "unit": "kg/m^3", "unitDescription": "kilograms per cubic metre"}], "typeOfFlow": "Product flow", "classification": {"classHierarchy": "Holz / Holzböden / Parkett", "name": "OEKOBAU.DAT"}}, {"dataSetInternalID": 1, "referenceToFlowDataSet": {"shortDescription": [{"value": "Erneuerbare Primärenergie als Energieträger (PERE)", "lang": "de"}, {"value": "Renewable primary energy as energy carrier (PERE)", "lang": "en"}], "type": "flow data set", "refObjectId": "20f32be5-0398-4288-9b6d-accddd195317", "uri": "../flows/20f32be5-0398-4288-9b6d-accddd195317.xml"}, "exchange direction": "INPUT", "other": {"anies": [{"name": "referenceToUnitGroupDataSet", "value": {"shortDescription": [{"value": "MJ", "lang": "de"}], "type": "unit group data set", "refObjectId": "93a60a57-a3c8-11da-a746-0800200c9a66", "uri": "../unitgroups/93a60a57-a3c8-11da-a746-0800200c9a66.xml"}}, {"value": "142.701897241884", "module": "A1-A3"}, {"value": "0.02115", "module": "A5"}, {"value": "41.28", "module": "B2"}, {"value": "3.025", "module": "B5"}, {"value": "0", "module": "C1"}, {"value": "0.0939", "module": "C2"}, {"value": "178.555512135556", "module": "C3", "scenario": "S1"}, {"value": "0.3133", "module": "C3", "scenario": "S2"}, {"value": "0", "module": "C4"}, {"value": "-27.04", "module": "D", "scenario": "S1"}, {"value": "-47.22", "module": "D", "scenario": "S2"}]}, "resolvedFlowVersion": "38.00.000", "flowProperties": [], "typeOfFlow": "Other flow", "classification": {"classHierarchy": "Quantities", "name": "GaBiCategories"}}, {"dataSetInternalID": 2, "referenceToFlowDataSet": {"shortDescription": [{"value": "Erneuerbare Primärenergie zur stofflichen Nutzung (PERM)", "lang": "de"}, {"value": "Renewable primary energy resources as material utilization (PERM)", "lang": "en"}], "type": "flow data set", "refObjectId": "fb3ec0de-548d-4508-aea5-00b73bf6f702", "uri": "../flows/fb3ec0de-548d-4508-aea5-00b73bf6f702.xml"}, "exchange direction": "INPUT", "other": {"anies": [{"name": "referenceToUnitGroupDataSet", "value": {"shortDescription": [{"value": "MJ", "lang": "de"}], "type": "unit group data set", "refObjectId": "93a60a57-a3c8-11da-a746-0800200c9a66", "uri": "../unitgroups/93a60a57-a3c8-11da-a746-0800200c9a66.xml"}}, {"value": "182.198102758116", "module": "A1-A3"}, {"value": "0", "module": "A5"}, {"value": "0", "module": "B2"}, {"value": "0", "module": "B5"}, {"value": "0", "module": "C1"}, {"value": "0", "module": "C2"}, {"value": "-177.752012135556", "module": "C3", "scenario": "S1"}, {"value": "0", "module": "C3", "scenario": "S2"}, {"value": "0", "module": "C4"}, {"value": "0", "module": "D", "scenario": "S1"}, {"value": "0", "module": "D", "scenario": "S2"}]}, "resolvedFlowVersion": "38.00.000", "flowProperties": [], "typeOfFlow": "Other flow", "classification": {"classHierarchy": "Quantities", "name": "GaBiCategories"}}, {"dataSetInternalID": 3, "referenceToFlowDataSet": {"shortDescription": [{"value": "Total erneuerbare Primärenergie (PERT)", "lang": "de"}, {"value": "Total use of renewable primary energy resources (PERT)", "lang": "en"}], "type": "flow data set", "refObjectId": "53f97275-fa8a-4cdd-9024-65936002acd0", "uri": "../flows/53f97275-fa8a-4cdd-9024-65936002acd0.xml"}, "exchange direction": "INPUT", "other": {"anies": [{"name": "referenceToUnitGroupDataSet", "value": {"shortDescription": [{"value": "MJ", "lang": "de"}], "type": "unit group data set", "refObjectId": "93a60a57-a3c8-11da-a746-0800200c9a66", "uri": "../unitgroups/93a60a57-a3c8-11da-a746-0800200c9a66.xml"}}, {"value": "324.9", "module": "A1-A3"}, {"value": "0.02115", "module": "A5"}, {"value": "41.28", "module": "B2"}, {"value": "3.025", "module": "B5"}, {"value": "0", "module": "C1"}, {"value": "0.0939", "module": "C2"}, {"value": "0.8035", "module": "C3", "scenario": "S1"}, {"value": "0.3133", "module": "C3", "scenario": "S2"}, {"value": "0", "module": "C4"}, {"value": "-27.04", "module": "D", "scenario": "S1"}, {"value": "-47.22", "module": "D", "scenario": "S2"}]}, "resolvedFlowVersion": "38.00.000", "flowProperties": [], "typeOfFlow": "Other flow", "classification": {"classHierarchy": "Quantities / Environmental quantities / EPD EN 15804 / LCI indicators", "name": "GaBiCategories"}}, {"dataSetInternalID": 4, "referenceToFlowDataSet": {"shortDescription": [{"value": "Nicht-erneuerbare Primärenergie als Energieträger (PENRE)", "lang": "de"}, {"value": "Non renewable primary energy as energy carrier (PENRE)", "lang": "en"}], "type": "flow data set", "refObjectId": "ac857178-2b45-46ec-892a-a9a4332f0372", "uri": "../flows/ac857178-2b45-46ec-892a-a9a4332f0372.xml"}, "exchange direction": "INPUT", "other": {"anies": [{"name": "referenceToUnitGroupDataSet", "value": {"shortDescription": [{"value": "MJ", "lang": "de"}], "type": "unit group data set", "refObjectId": "93a60a57-a3c8-11da-a746-0800200c9a66", "uri": "../unitgroups/93a60a57-a3c8-11da-a746-0800200c9a66.xml"}}, {"value": "171.6913586642", "module": "A1-A3"}, {"value": "0.1401", "module": "A5"}, {"value": "97.67", "module": "B2"}, {"value": "15.48", "module": "B5"}, {"value": "0", "module": "C1"}, {"value": "1.638", "module": "C2"}, {"value": "9.689", "module": "C3", "scenario": "S1"}, {"value": "2.125", "module": "C3", "scenario": "S2"}, {"value": "0", "module": "C4"}, {"value": "-119.1", "module": "D", "scenario": "S1"}, {"value": "-5.065", "module": "D", "scenario": "S2"}]}, "resolvedFlowVersion": "38.00.000", "flowProperties": [], "typeOfFlow": "Other flow", "classification": {"classHierarchy": "Quantities", "name": "GaBiCategories"}}, {"dataSetInternalID": 5, "referenceToFlowDataSet": {"shortDescription": [{"value": "Nicht-erneuerbare Primärenergie zur stofflichen Nutzung (PENRM)", "lang": "de"}, {"value": "Non renewable primary energy as material utilization (PENRM)", "lang": "en"}], "type": "flow data set", "refObjectId": "1421caa0-679d-4bf4-b282-0eb850ccae27", "uri": "../flows/1421caa0-679d-4bf4-b282-0eb850ccae27.xml"}, "exchange direction": "INPUT", "other": {"anies": [{"name": "referenceToUnitGroupDataSet", "value": {"shortDescription": [{"value": "MJ", "lang": "de"}], "type": "unit group data set", "refObjectId": "93a60a57-a3c8-11da-a746-0800200c9a66", "uri": "../unitgroups/93a60a57-a3c8-11da-a746-0800200c9a66.xml"}}, {"value": "6.8086413358", "module": "A1-A3"}, {"value": "0", "module": "A5"}, {"value": "0", "module": "B2"}, {"value": "0", "module": "B5"}, {"value": "0", "module": "C1"}, {"value": "0", "module": "C2"}, {"value": "-5.544", "module": "C3", "scenario": "S1"}, {"value": "0", "module": "C3", "scenario": "S2"}, {"value": "0", "module": "C4"}, {"value": "0", "module": "D", "scenario": "S1"}, {"value": "0", "module": "D", "scenario": "S2"}]}, "resolvedFlowVersion": "38.00.000", "flowProperties": [], "typeOfFlow": "Other flow", "classification": {"classHierarchy": "Quantities", "name": "GaBiCategories"}}, {"dataSetInternalID": 6, "referenceToFlowDataSet": {"shortDescription": [{"value": "Total nicht erneuerbare Primärenergie (PENRT)", "lang": "de"}, {"value": "Total use of non renewable primary energy resources (PENRT)", "lang": "en"}], "type": "flow data set", "refObjectId": "06159210-646b-4c8d-8583-da9b3b95a6c1", "uri": "../flows/06159210-646b-4c8d-8583-da9b3b95a6c1.xml"}, "exchange direction": "INPUT", "other": {"anies": [{"name": "referenceToUnitGroupDataSet", "value": {"shortDescription": [{"value": "MJ", "lang": "de"}], "type": "unit group data set", "refObjectId": "93a60a57-a3c8-11da-a746-0800200c9a66", "uri": "../unitgroups/93a60a57-a3c8-11da-a746-0800200c9a66.xml"}}, {"value": "178.5", "module": "A1-A3"}, {"value": "0.1401", "module": "A5"}, {"value": "97.67", "module": "B2"}, {"value": "15.48", "module": "B5"}, {"value": "0", "module": "C1"}, {"value": "1.638", "module": "C2"}, {"value": "4.145", "module": "C3", "scenario": "S1"}, {"value": "2.125", "module": "C3", "scenario": "S2"}, {"value": "0", "module": "C4"}, {"value": "-119.1", "module": "D", "scenario": "S1"}, {"value": "-5.065", "module": "D", "scenario": "S2"}]}, "resolvedFlowVersion": "38.00.000", "flowProperties": [], "typeOfFlow": "Other flow", "classification": {"classHierarchy": "Quantities / Environmental quantities / EPD EN 15804 / LCI indicators", "name": "GaBiCategories"}}, {"dataSetInternalID": 7, "referenceToFlowDataSet": {"shortDescription": [{"value": "Einsatz von Sekundärstoffen (SM)", "lang": "de"}, {"value": "Use of secondary material (SM)", "lang": "en"}], "type": "flow data set", "refObjectId": "c6a1f35f-2d09-4f54-8dfb-97e502e1ce92", "uri": "../flows/c6a1f35f-2d09-4f54-8dfb-97e502e1ce92.xml"}, "exchange direction": "INPUT", "other": {"anies": [{"name": "referenceToUnitGroupDataSet", "value": {"shortDescription": [{"value": "kg", "lang": "de"}], "type": "unit group data set", "refObjectId": "ad38d542-3fe9-439d-9b95-2f5f7752acaf", "uri": "../unitgroups/ad38d542-3fe9-439d-9b95-2f5f7752acaf.xml"}}, {"value": "0", "module": "A1-A3"}, {"value": "0", "module": "A5"}, {"value": "0", "module": "B2"}, {"value": "0", "module": "B5"}, {"value": "0", "module": "C1"}, {"value": "0", "module": "C2"}, {"value": "0", "module": "C3", "scenario": "S1"}, {"value": "0", "module": "C3", "scenario": "S2"}, {"value": "0", "module": "C4"}, {"value": "0", "module": "D", "scenario": "S1"}, {"value": "0", "module": "D", "scenario": "S2"}]}, "resolvedFlowVersion": "38.00.000", "flowProperties": [], "typeOfFlow": "Other flow", "classification": {"classHierarchy": "Quantities / Environmental quantities / EPD EN 15804 / LCI indicators", "name": "GaBiCategories"}}, {"dataSetInternalID": 8, "referenceToFlowDataSet": {"shortDescription": [{"value": "Erneuerbare Sekundärbrennstoffe (RSF)", "lang": "de"}, {"value": "Use of renewable secondary fuels (RSF)", "lang": "en"}], "type": "flow data set", "refObjectId": "64333088-a55f-4aa2-9a31-c10b07816787", "uri": "../flows/64333088-a55f-4aa2-9a31-c10b07816787.xml"}, "exchange direction": "INPUT", "other": {"anies": [{"name": "referenceToUnitGroupDataSet", "value": {"shortDescription": [{"value": "MJ", "lang": "de"}], "type": "unit group data set", "refObjectId": "93a60a57-a3c8-11da-a746-0800200c9a66", "uri": "../unitgroups/93a60a57-a3c8-11da-a746-0800200c9a66.xml"}}, {"value": "0", "module": "A1-A3"}, {"value": "0", "module": "A5"}, {"value": "0", "module": "B2"}, {"value": "0", "module": "B5"}, {"value": "0", "module": "C1"}, {"value": "0", "module": "C2"}, {"value": "0", "module": "C3", "scenario": "S1"}, {"value": "0", "module": "C3", "scenario": "S2"}, {"value": "0", "module": "C4"}, {"value": "177.752012135556", "module": "D", "scenario": "S1"}, {"value": "0", "module": "D", "scenario": "S2"}]}, "resolvedFlowVersion": "38.00.000", "flowProperties": [], "typeOfFlow": "Other flow", "classification": {"classHierarchy": "Quantities / Environmental quantities / EPD EN 15804 / LCI indicators", "name": "GaBiCategories"}}, {"dataSetInternalID": 9, "referenceToFlowDataSet": {"shortDescription": [{"value": "Nicht erneuerbare Sekundärbrennstoffe (NRSF)", "lang": "de"}, {"value": "Use of non renewable secondary fuels (NRSF)", "lang": "en"}], "type": "flow data set", "refObjectId": "89def144-d39a-4287-b86f-efde453ddcb2", "uri": "../flows/89def144-d39a-4287-b86f-efde453ddcb2.xml"}, "exchange direction": "INPUT", "other": {"anies": [{"name": "referenceToUnitGroupDataSet", "value": {"shortDescription": [{"value": "MJ", "lang": "de"}], "type": "unit group data set", "refObjectId": "93a60a57-a3c8-11da-a746-0800200c9a66", "uri": "../unitgroups/93a60a57-a3c8-11da-a746-0800200c9a66.xml"}}, {"value": "0", "module": "A1-A3"}, {"value": "0", "module": "A5"}, {"value": "0", "module": "B2"}, {"value": "0", "module": "B5"}, {"value": "0", "module": "C1"}, {"value": "0", "module": "C2"}, {"value": "0", "module": "C3", "scenario": "S1"}, {"value": "0", "module": "C3", "scenario": "S2"}, {"value": "0", "module": "C4"}, {"value": "0", "module": "D", "scenario": "S1"}, {"value": "0", "module": "D", "scenario": "S2"}]}, "resolvedFlowVersion": "38.00.000", "flowProperties": [], "typeOfFlow": "Other flow", "classification": {"classHierarchy": "Quantities / Environmental quantities / EPD EN 15804 / LCI indicators", "name": "GaBiCategories"}}, {"dataSetInternalID": 10, "referenceToFlowDataSet": {"shortDescription": [{"value": "Einsatz von Süßwasserressourcen (FW)", "lang": "de"}, {"value": "Use of net fresh water (FW)", "lang": "en"}], "type": "flow data set", "refObjectId": "3cf952c8-f3a4-461d-8c96-96456ca62246", "uri": "../flows/3cf952c8-f3a4-461d-8c96-96456ca62246.xml"}, "exchange direction": "INPUT", "other": {"anies": [{"name": "referenceToUnitGroupDataSet", "value": {"shortDescription": [{"value": "m^3", "lang": "de"}], "type": "unit group data set", "refObjectId": "cd950537-0a98-4044-9ba7-9f9a68d0a504", "uri": "../unitgroups/cd950537-0a98-4044-9ba7-9f9a68d0a504.xml"}}, {"value": "0.05476", "module": "A1-A3"}, {"value": "0.001146", "module": "A5"}, {"value": "0.04189", "module": "B2"}, {"value": "0.007271", "module": "B5"}, {"value": "0", "module": "C1"}, {"value": "0.0001075", "module": "C2"}, {"value": "0.04634", "module": "C3", "scenario": "S1"}, {"value": "0.001559", "module": "C3", "scenario": "S2"}, {"value": "0", "module": "C4"}, {"value": "-0.02641", "module": "D", "scenario": "S1"}, {"value": "-0.001957", "module": "D", "scenario": "S2"}]}, "resolvedFlowVersion": "38.00.000", "flowProperties": [], "typeOfFlow": "Other flow", "classification": {"classHierarchy": "Quantities / Environmental quantities / EPD EN 15804 / LCI indicators", "name": "GaBiCategories"}}, {"dataSetInternalID": 11, "referenceToFlowDataSet": {"shortDescription": [{"value": "Gefährlicher Abfall zur Deponie (HWD)", "lang": "de"}, {"value": "Hazardous waste disposed (HWD)", "lang": "en"}], "type": "flow data set", "refObjectId": "430f9e0f-59b2-46a0-8e0d-55e0e84948fc", "uri": "../flows/430f9e0f-59b2-46a0-8e0d-55e0e84948fc.xml"}, "exchange direction": "OUTPUT", "other": {"anies": [{"name": "referenceToUnitGroupDataSet", "value": {"shortDescription": [{"value": "kg", "lang": "de"}], "type": "unit group data set", "refObjectId": "ad38d542-3fe9-439d-9b95-2f5f7752acaf", "uri": "../unitgroups/ad38d542-3fe9-439d-9b95-2f5f7752acaf.xml"}}, {"value": "3.295E-07", "module": "A1-A3"}, {"value": "1.959E-11", "module": "A5"}, {"value": "2.413E-08", "module": "B2"}, {"value": "3.175E-09", "module": "B5"}, {"value": "0", "module": "C1"}, {"value": "8.629E-11", "module": "C2"}, {"value": "7.479E-10", "module": "C3", "scenario": "S1"}, {"value": "0", "module": "C3", "scenario": "S2"}, {"value": "0", "module": "C4"}, {"value": "-2.679E-08", "module": "D", "scenario": "S1"}, {"value": "0", "module": "D", "scenario": "S2"}]}, "resolvedFlowVersion": "38.00.000", "flowProperties": [], "typeOfFlow": "Other flow", "classification": {"classHierarchy": "Quantities / Environmental quantities / EPD EN 15804 / LCI indicators", "name": "GaBiCategories"}}, {"dataSetInternalID": 12, "referenceToFlowDataSet": {"shortDescription": [{"value": "Entsorgter nicht gefährlicher Abfall (NHWD)", "lang": "de"}, {"value": "Non hazardous waste disposed (NHWD)", "lang": "en"}], "type": "flow data set", "refObjectId": "b29ef66b-e286-4afa-949f-62f1a7b4d7fa", "uri": "../flows/b29ef66b-e286-4afa-949f-62f1a7b4d7fa.xml"}, "exchange direction": "OUTPUT", "other": {"anies": [{"name": "referenceToUnitGroupDataSet", "value": {"shortDescription": [{"value": "kg", "lang": "de"}], "type": "unit group data set", "refObjectId": "ad38d542-3fe9-439d-9b95-2f5f7752acaf", "uri": "../unitgroups/ad38d542-3fe9-439d-9b95-2f5f7752acaf.xml"}}, {"value": "0.2152", "module": "A1-A3"}, {"value": "0.003163", "module": "A5"}, {"value": "0.2636", "module": "B2"}, {"value": "0.02222", "module": "B5"}, {"value": "0", "module": "C1"}, {"value": "0.0002569", "module": "C2"}, {"value": "0.1369", "module": "C3", "scenario": "S1"}, {"value": "0", "module": "C3", "scenario": "S2"}, {"value": "0", "module": "C4"}, {"value": "-0.05602", "module": "D", "scenario": "S1"}, {"value": "0", "module": "D", "scenario": "S2"}]}, "resolvedFlowVersion": "38.00.000", "flowProperties": [], "typeOfFlow": "Other flow", "classification": {"classHierarchy": "Quantities / Environmental quantities / EPD EN 15804 / LCI indicators", "name": "GaBiCategories"}}, {"dataSetInternalID": 13, "referenceToFlowDataSet": {"shortDescription": [{"value": "Entsorgter radioaktiver Abfall (RWD)", "lang": "de"}, {"value": "Radioactive waste disposed (RWD)", "lang": "en"}], "type": "flow data set", "refObjectId": "3449546e-52ad-4b39-b809-9fb77cea8ff6", "uri": "../flows/3449546e-52ad-4b39-b809-9fb77cea8ff6.xml"}, "exchange direction": "OUTPUT", "other": {"anies": [{"name": "referenceToUnitGroupDataSet", "value": {"shortDescription": [{"value": "kg", "lang": "de"}], "type": "unit group data set", "refObjectId": "ad38d542-3fe9-439d-9b95-2f5f7752acaf", "uri": "../unitgroups/ad38d542-3fe9-439d-9b95-2f5f7752acaf.xml"}}, {"value": "0.007443", "module": "A1-A3"}, {"value": "5.407E-06", "module": "A5"}, {"value": "0.01332", "module": "B2"}, {"value": "0.0008954", "module": "B5"}, {"value": "0", "module": "C1"}, {"value": "2.971E-06", "module": "C2"}, {"value": "0.0002299", "module": "C3", "scenario": "S1"}, {"value": "0", "module": "C3", "scenario": "S2"}, {"value": "0", "module": "C4"}, {"value": "-0.0087", "module": "D", "scenario": "S1"}, {"value": "0", "module": "D", "scenario": "S2"}]}, "resolvedFlowVersion": "38.00.000", "flowProperties": [], "typeOfFlow": "Other flow", "classification": {"classHierarchy": "Quantities / Environmental quantities / EPD EN 15804 / LCI indicators", "name": "GaBiCategories"}}, {"dataSetInternalID": 14, "referenceToFlowDataSet": {"shortDescription": [{"value": "Komponenten für die Wiederverwendung (CRU)", "lang": "de"}, {"value": "Components for re-use (CRU)", "lang": "en"}], "type": "flow data set", "refObjectId": "a2b32f97-3fc7-4af2-b209-525bc6426f33", "uri": "../flows/a2b32f97-3fc7-4af2-b209-525bc6426f33.xml"}, "exchange direction": "OUTPUT", "other": {"anies": [{"name": "referenceToUnitGroupDataSet", "value": {"shortDescription": [{"value": "kg", "lang": "de"}], "type": "unit group data set", "refObjectId": "ad38d542-3fe9-439d-9b95-2f5f7752acaf", "uri": "../unitgroups/ad38d542-3fe9-439d-9b95-2f5f7752acaf.xml"}}, {"value": "0", "module": "A1-A3"}, {"value": "0", "module": "A5"}, {"value": "0", "module": "B2"}, {"value": "0", "module": "B5"}, {"value": "0", "module": "C1"}, {"value": "0", "module": "C2"}, {"value": "0", "module": "C3", "scenario": "S1"}, {"value": "0", "module": "C3", "scenario": "S2"}, {"value": "0", "module": "C4"}, {"value": "0", "module": "D", "scenario": "S1"}, {"value": "0", "module": "D", "scenario": "S2"}]}, "resolvedFlowVersion": "38.00.000", "flowProperties": [], "typeOfFlow": "Other flow", "classification": {"classHierarchy": "Quantities / Environmental quantities / EPD EN 15804 / LCI indicators", "name": "GaBiCategories"}}, {"dataSetInternalID": 15, "referenceToFlowDataSet": {"shortDescription": [{"value": "Stoffe zum Recycling (MFR)", "lang": "de"}, {"value": "Materials for recycling (MFR)", "lang": "en"}], "type": "flow data set", "refObjectId": "d7fe48a5-4103-49c8-9aae-b0b5dfdbd6ae", "uri": "../flows/d7fe48a5-4103-49c8-9aae-b0b5dfdbd6ae.xml"}, "exchange direction": "OUTPUT", "other": {"anies": [{"name": "referenceToUnitGroupDataSet", "value": {"shortDescription": [{"value": "kg", "lang": "de"}], "type": "unit group data set", "refObjectId": "ad38d542-3fe9-439d-9b95-2f5f7752acaf", "uri": "../unitgroups/ad38d542-3fe9-439d-9b95-2f5f7752acaf.xml"}}, {"value": "0", "module": "A1-A3"}, {"value": "0.04113", "module": "A5"}, {"value": "0", "module": "B2"}, {"value": "0", "module": "B5"}, {"value": "0", "module": "C1"}, {"value": "0", "module": "C2"}, {"value": "0", "module": "C3", "scenario": "S1"}, {"value": "0", "module": "C3", "scenario": "S2"}, {"value": "0", "module": "C4"}, {"value": "0", "module": "D", "scenario": "S1"}, {"value": "0", "module": "D", "scenario": "S2"}]}, "resolvedFlowVersion": "38.00.000", "flowProperties": [], "typeOfFlow": "Other flow", "classification": {"classHierarchy": "Quantities / Environmental quantities / EPD EN 15804 / LCI indicators", "name": "GaBiCategories"}}, {"dataSetInternalID": 16, "referenceToFlowDataSet": {"shortDescription": [{"value": "Stoffe für die Energierückgewinnung (MER)", "lang": "de"}, {"value": "Materials for energy recovery (MER)", "lang": "en"}], "type": "flow data set", "refObjectId": "59a9181c-3aaf-46ee-8b13-2b3723b6e447", "uri": "../flows/59a9181c-3aaf-46ee-8b13-2b3723b6e447.xml"}, "exchange direction": "OUTPUT", "other": {"anies": [{"name": "referenceToUnitGroupDataSet", "value": {"shortDescription": [{"value": "kg", "lang": "de"}], "type": "unit group data set", "refObjectId": "ad38d542-3fe9-439d-9b95-2f5f7752acaf", "uri": "../unitgroups/ad38d542-3fe9-439d-9b95-2f5f7752acaf.xml"}}, {"value": "1.016", "module": "A1-A3"}, {"value": "0.2441", "module": "A5"}, {"value": "0.06338", "module": "B2"}, {"value": "0.484", "module": "B5"}, {"value": "0", "module": "C1"}, {"value": "0", "module": "C2"}, {"value": "10.53", "module": "C3", "scenario": "S1"}, {"value": "0", "module": "C3", "scenario": "S2"}, {"value": "0", "module": "C4"}, {"value": "0", "module": "D", "scenario": "S1"}, {"value": "0", "module": "D", "scenario": "S2"}]}, "resolvedFlowVersion": "38.00.000", "flowProperties": [], "typeOfFlow": "Other flow", "classification": {"classHierarchy": "Quantities / Environmental quantities / EPD EN 15804 / LCI indicators", "name": "GaBiCategories"}}, {"dataSetInternalID": 17, "referenceToFlowDataSet": {"shortDescription": [{"value": "Exportierte elektrische Energie (EEE)", "lang": "de"}, {"value": "Exported electrical energy (EEE)", "lang": "en"}], "type": "flow data set", "refObjectId": "4da0c987-2b76-40d6-9e9e-82a017aaaf29", "uri": "../flows/4da0c987-2b76-40d6-9e9e-82a017aaaf29.xml"}, "exchange direction": "OUTPUT", "other": {"anies": [{"name": "referenceToUnitGroupDataSet", "value": {"shortDescription": [{"value": "MJ", "lang": "de"}], "type": "unit group data set", "refObjectId": "93a60a57-a3c8-11da-a746-0800200c9a66", "uri": "../unitgroups/93a60a57-a3c8-11da-a746-0800200c9a66.xml"}}, {"value": "0", "module": "A1-A3"}, {"value": "0.7576", "module": "A5"}, {"value": "0", "module": "B2"}, {"value": "1.355", "module": "B5"}, {"value": "0", "module": "C1"}, {"value": "0", "module": "C2"}, {"value": "27.55", "module": "C3", "scenario": "S1"}, {"value": "0", "module": "C3", "scenario": "S2"}, {"value": "0", "module": "C4"}, {"value": "0", "module": "D", "scenario": "S1"}, {"value": "0", "module": "D", "scenario": "S2"}]}, "resolvedFlowVersion": "38.00.000", "flowProperties": [], "typeOfFlow": "Other flow", "classification": {"classHierarchy": "Quantities / Environmental quantities / EPD EN 15804 / LCI indicators", "name": "GaBiCategories"}}, {"dataSetInternalID": 18, "referenceToFlowDataSet": {"shortDescription": [{"value": "Exportierte thermische Energie (EET)", "lang": "de"}, {"value": "Exported thermal energy (EET)", "lang": "en"}], "type": "flow data set", "refObjectId": "98daf38a-7a79-46d3-9a37-2b7bd0955810", "uri": "../flows/98daf38a-7a79-46d3-9a37-2b7bd0955810.xml"}, "exchange direction": "OUTPUT", "other": {"anies": [{"name": "referenceToUnitGroupDataSet", "value": {"shortDescription": [{"value": "MJ", "lang": "de"}], "type": "unit group data set", "refObjectId": "93a60a57-a3c8-11da-a746-0800200c9a66", "uri": "../unitgroups/93a60a57-a3c8-11da-a746-0800200c9a66.xml"}}, {"value": "0", "module": "A1-A3"}, {"value": "1.357", "module": "A5"}, {"value": "0", "module": "B2"}, {"value": "2.441", "module": "B5"}, {"value": "0", "module": "C1"}, {"value": "0", "module": "C2"}, {"value": "49.49", "module": "C3", "scenario": "S1"}, {"value": "0", "module": "C3", "scenario": "S2"}, {"value": "0", "module": "C4"}, {"value": "0", "module": "D", "scenario": "S1"}, {"value": "0", "module": "D", "scenario": "S2"}]}, "resolvedFlowVersion": "38.00.000", "flowProperties": [], "typeOfFlow": "Other flow", "classification": {"classHierarchy": "Quantities / Environmental quantities / EPD EN 15804 / LCI indicators", "name": "GaBiCategories"}}]}, "LCIAResults": {"LCIAResult": [{"referenceToLCIAMethodDataSet": {"shortDescription": [{"value": "Globales Erwärmungspotenzial total (GWP-total)", "lang": "de"}, {"value": "Global Warming Potential total (GWP-total)", "lang": "en"}], "type": "LCIA method data set", "refObjectId": "6a37f984-a4b3-458a-a20a-64418c145fa2", "uri": "../lciamethods/6a37f984-a4b3-458a-a20a-64418c145fa2.xml"}, "other": {"anies": [{"name": "referenceToUnitGroupDataSet", "value": {"shortDescription": [{"value": "kg CO_(2)-Äq.", "lang": "de"}], "type": "unit group data set", "refObjectId": "1ebf3012-d0db-4de2-aefd-ef30cedb0be1", "uri": "../unitgroups/1ebf3012-d0db-4de2-aefd-ef30cedb0be1.xml"}}, {"value": "-9.094", "module": "A1-A3"}, {"value": "0.4916", "module": "A5"}, {"value": "5.394", "module": "B2"}, {"value": "0.08573", "module": "B5"}, {"value": "0", "module": "C1"}, {"value": "0.1234", "module": "C2"}, {"value": "19.09", "module": "C3", "scenario": "S1"}, {"value": "18.15", "module": "C3", "scenario": "S2"}, {"value": "0", "module": "C4"}, {"value": "-6.867", "module": "D", "scenario": "S1"}, {"value": "-0.1666", "module": "D", "scenario": "S2"}]}}, {"referenceToLCIAMethodDataSet": {"shortDescription": [{"value": "Globales Erwärmungspotenzial fossil (GWP-fossil)", "lang": "de"}, {"value": "Global Warming Potential fossil fuels (GWP-fossil)", "lang": "en"}], "type": "LCIA method data set", "refObjectId": "5f635281-343e-44fb-83df-1971b155e6b6", "uri": "../lciamethods/5f635281-343e-44fb-83df-1971b155e6b6.xml"}, "other": {"anies": [{"name": "referenceToUnitGroupDataSet", "value": {"shortDescription": [{"value": "kg CO_(2)-Äq.", "lang": "de"}], "type": "unit group data set", "refObjectId": "1ebf3012-d0db-4de2-aefd-ef30cedb0be1", "uri": "../unitgroups/1ebf3012-d0db-4de2-aefd-ef30cedb0be1.xml"}}, {"value": "9.558", "module": "A1-A3"}, {"value": "0.1007", "module": "A5"}, {"value": "5.425", "module": "B2"}, {"value": "0.7317", "module": "B5"}, {"value": "0", "module": "C1"}, {"value": "0.1224", "module": "C2"}, {"value": "0.2815", "module": "C3", "scenario": "S1"}, {"value": "0.09212", "module": "C3", "scenario": "S2"}, {"value": "0", "module": "C4"}, {"value": "-6.863", "module": "D", "scenario": "S1"}, {"value": "-0.3292", "module": "D", "scenario": "S2"}]}}, {"referenceToLCIAMethodDataSet": {"shortDescription": [{"value": "Globales Erwärmungspotenzial biogen (GWP-biogenic)", "lang": "de"}, {"value": "Global Warming Potential biogenic (GWP-biogenic)", "lang": "en"}], "type": "LCIA method data set", "refObjectId": "2356e1ab-0185-4db5-86e5-16de51c7485c", "uri": "../lciamethods/2356e1ab-0185-4db5-86e5-16de51c7485c.xml"}, "other": {"anies": [{"name": "referenceToUnitGroupDataSet", "value": {"shortDescription": [{"value": "kg CO_(2)-Äq.", "lang": "de"}], "type": "unit group data set", "refObjectId": "1ebf3012-d0db-4de2-aefd-ef30cedb0be1", "uri": "../unitgroups/1ebf3012-d0db-4de2-aefd-ef30cedb0be1.xml"}}, {"value": "-18.68", "module": "A1-A3"}, {"value": "0.3908", "module": "A5"}, {"value": "0", "module": "B2"}, {"value": "-0.6466", "module": "B5"}, {"value": "0", "module": "C1"}, {"value": "0", "module": "C2"}, {"value": "18.81", "module": "C3", "scenario": "S1"}, {"value": "18.06", "module": "C3", "scenario": "S2"}, {"value": "0", "module": "C4"}, {"value": "0", "module": "D", "scenario": "S1"}, {"value": "0", "module": "D", "scenario": "S2"}]}}, {"referenceToLCIAMethodDataSet": {"shortDescription": [{"value": "Globales Erwärmungspotenzial luluc (GWP-luluc)", "lang": "de"}, {"value": "Global Warming Potential luluc (GWP-luluc)", "lang": "en"}], "type": "LCIA method data set", "refObjectId": "4331bbdb-978a-490d-8707-eeb047f01a55", "uri": "../lciamethods/4331bbdb-978a-490d-8707-eeb047f01a55.xml"}, "other": {"anies": [{"name": "referenceToUnitGroupDataSet", "value": {"shortDescription": [{"value": "kg CO_(2)-Äq.", "lang": "de"}], "type": "unit group data set", "refObjectId": "1ebf3012-d0db-4de2-aefd-ef30cedb0be1", "uri": "../unitgroups/1ebf3012-d0db-4de2-aefd-ef30cedb0be1.xml"}}, {"value": "0.02405", "module": "A1-A3"}, {"value": "3.13E-05", "module": "A5"}, {"value": "0.00718", "module": "B2"}, {"value": "0.0006111", "module": "B5"}, {"value": "0", "module": "C1"}, {"value": "0.001001", "module": "C2"}, {"value": "0.0001807", "module": "C3", "scenario": "S1"}, {"value": "0.0002074", "module": "C3", "scenario": "S2"}, {"value": "0", "module": "C4"}, {"value": "-0.004761", "module": "D", "scenario": "S1"}, {"value": "-0.001832", "module": "D", "scenario": "S2"}]}}, {"referenceToLCIAMethodDataSet": {"shortDescription": [{"value": "Abbau Potential der stratosphärischen Ozonschicht (ODP)", "lang": "de"}, {"value": "Depletion potential of the stratospheric ozone layer (ODP)", "lang": "en"}], "type": "LCIA method data set", "refObjectId": "b5c629d6-def3-11e6-bf01-fe55135034f3", "uri": "../lciamethods/b5c629d6-def3-11e6-bf01-fe55135034f3.xml"}, "other": {"anies": [{"name": "referenceToUnitGroupDataSet", "value": {"shortDescription": [{"value": "kg CFC11-Äq.", "lang": "de"}], "type": "unit group data set", "refObjectId": "d9e957c9-7309-4474-bf3a-7777df6c4e5b", "uri": "../unitgroups/d9e957c9-7309-4474-bf3a-7777df6c4e5b.xml"}}, {"value": "1.92E-08", "module": "A1-A3"}, {"value": "5.848E-17", "module": "A5"}, {"value": "1.206E-13", "module": "B2"}, {"value": "8.303E-15", "module": "B5"}, {"value": "0", "module": "C1"}, {"value": "2.419E-17", "module": "C2"}, {"value": "2.498E-15", "module": "C3", "scenario": "S1"}, {"value": "7.707E-09", "module": "C3", "scenario": "S2"}, {"value": "0", "module": "C4"}, {"value": "-7.87E-14", "module": "D", "scenario": "S1"}, {"value": "-2.772E-08", "module": "D", "scenario": "S2"}]}}, {"referenceToLCIAMethodDataSet": {"shortDescription": [{"value": "Versauerungspotenzial von Boden und Wasser (AP)", "lang": "de"}, {"value": "Acidification potential of land and water (AP)", "lang": "en"}], "type": "LCIA method data set", "refObjectId": "b5c611c6-def3-11e6-bf01-fe55135034f3", "uri": "../lciamethods/b5c611c6-def3-11e6-bf01-fe55135034f3.xml"}, "other": {"anies": [{"name": "referenceToUnitGroupDataSet", "value": {"shortDescription": [{"value": "mol H^(+)-Äq.", "lang": "de"}], "type": "unit group data set", "refObjectId": "42e089ac-92bf-4bf2-8ca1-5fc40d18f2ed", "uri": "../unitgroups/42e089ac-92bf-4bf2-8ca1-5fc40d18f2ed.xml"}}, {"value": "0.0305", "module": "A1-A3"}, {"value": "6.828E-05", "module": "A5"}, {"value": "0.01111", "module": "B2"}, {"value": "0.001448", "module": "B5"}, {"value": "0", "module": "C1"}, {"value": "0.0001426", "module": "C2"}, {"value": "0.002709", "module": "C3", "scenario": "S1"}, {"value": "0.0005088", "module": "C3", "scenario": "S2"}, {"value": "0", "module": "C4"}, {"value": "-0.008986", "module": "D", "scenario": "S1"}, {"value": "-0.001836", "module": "D", "scenario": "S2"}]}}, {"referenceToLCIAMethodDataSet": {"shortDescription": [{"value": "Eutrophierungspotenzial Süßwasser (EP-freshwater)", "lang": "de"}, {"value": "Eutrophication potential aquatic freshwater (EP-freshwater)", "lang": "en"}], "type": "LCIA method data set", "refObjectId": "b53ec18f-7377-4ad3-86eb-cc3f4f276b2b", "uri": "../lciamethods/b53ec18f-7377-4ad3-86eb-cc3f4f276b2b.xml"}, "other": {"anies": [{"name": "referenceToUnitGroupDataSet", "value": {"shortDescription": [{"value": "kg PO_(4)-Äq.", "lang": "de"}], "type": "unit group data set", "refObjectId": "0429039d-a61d-4590-ba67-aa4a20a810a1", "uri": "../unitgroups/0429039d-a61d-4590-ba67-aa4a20a810a1.xml"}}, {"value": "9.073E-05", "module": "A1-A3"}, {"value": "1.776E-08", "module": "A5"}, {"value": "0.0001353", "module": "B2"}, {"value": "1.578E-06", "module": "B5"}, {"value": "0", "module": "C1"}, {"value": "3.64E-07", "module": "C2"}, {"value": "3.424E-07", "module": "C3", "scenario": "S1"}, {"value": "8.85E-05", "module": "C3", "scenario": "S2"}, {"value": "0", "module": "C4"}, {"value": "-9.004E-06", "module": "D", "scenario": "S1"}, {"value": "-0.000138", "module": "D", "scenario": "S2"}]}}, {"referenceToLCIAMethodDataSet": {"shortDescription": [{"value": "Eutrophierungspotenzial Salzwasser (EP-marine)", "lang": "de"}, {"value": "Eutrophication potential aquatic marine (EP-marine)", "lang": "en"}], "type": "LCIA method data set", "refObjectId": "b5c619fa-def3-11e6-bf01-fe55135034f3", "uri": "../lciamethods/b5c619fa-def3-11e6-bf01-fe55135034f3.xml"}, "other": {"anies": [{"name": "referenceToUnitGroupDataSet", "value": {"shortDescription": [{"value": "kg N-Äq.", "lang": "de"}], "type": "unit group data set", "refObjectId": "d05bb823-ecdf-4686-8c40-bf1d9257859f", "uri": "../unitgroups/d05bb823-ecdf-4686-8c40-bf1d9257859f.xml"}}, {"value": "0.01306", "module": "A1-A3"}, {"value": "2.137E-05", "module": "A5"}, {"value": "0.003111", "module": "B2"}, {"value": "0.0003763", "module": "B5"}, {"value": "0", "module": "C1"}, {"value": "4.785E-05", "module": "C2"}, {"value": "0.00089", "module": "C3", "scenario": "S1"}, {"value": "8.801E-05", "module": "C3", "scenario": "S2"}, {"value": "0", "module": "C4"}, {"value": "-0.002552", "module": "D", "scenario": "S1"}, {"value": "-0.0004687", "module": "D", "scenario": "S2"}]}}, {"referenceToLCIAMethodDataSet": {"shortDescription": [{"value": "Eutrophierungspotenzial Land (EP-terrestrial)", "lang": "de"}, {"value": "Eutrophication potential terrestrial (EP-terrestrial)", "lang": "en"}], "type": "LCIA method data set", "refObjectId": "b5c614d2-def3-11e6-bf01-fe55135034f3", "uri": "../lciamethods/b5c614d2-def3-11e6-bf01-fe55135034f3.xml"}, "other": {"anies": [{"name": "referenceToUnitGroupDataSet", "value": {"shortDescription": [{"value": "mol N-Äq.", "lang": "de"}], "type": "unit group data set", "refObjectId": "71b4d617-0ec9-4d3f-b65e-e438940c2401", "uri": "../unitgroups/71b4d617-0ec9-4d3f-b65e-e438940c2401.xml"}}, {"value": "0.1191", "module": "A1-A3"}, {"value": "0.0003216", "module": "A5"}, {"value": "0.02799", "module": "B2"}, {"value": "0.004168", "module": "B5"}, {"value": "0", "module": "C1"}, {"value": "0.0005645", "module": "C2"}, {"value": "0.01291", "module": "C3", "scenario": "S1"}, {"value": "0.0008341", "module": "C3", "scenario": "S2"}, {"value": "0", "module": "C4"}, {"value": "-0.02734", "module": "D", "scenario": "S1"}, {"value": "-0.004886", "module": "D", "scenario": "S2"}]}}, {"referenceToLCIAMethodDataSet": {"shortDescription": [{"value": "Bildungspotential für troposphärisches Ozon (POCP)", "lang": "de"}, {"value": "Formation potential of tropospheric ozone photochemical oxidants (POCP)", "lang": "en"}], "type": "LCIA method data set", "refObjectId": "b5c610fe-def3-11e6-bf01-fe55135034f3", "uri": "../lciamethods/b5c610fe-def3-11e6-bf01-fe55135034f3.xml"}, "other": {"anies": [{"name": "referenceToUnitGroupDataSet", "value": {"shortDescription": [{"value": "kg NMVOC-Äq.", "lang": "de"}], "type": "unit group data set", "refObjectId": "d27c25f8-fbc1-44c6-b47b-4adbae4199c6", "uri": "../unitgroups/d27c25f8-fbc1-44c6-b47b-4adbae4199c6.xml"}}, {"value": "0.03702", "module": "A1-A3"}, {"value": "5.844E-05", "module": "A5"}, {"value": "0.00753", "module": "B2"}, {"value": "0.001179", "module": "B5"}, {"value": "0", "module": "C1"}, {"value": "0.0001254", "module": "C2"}, {"value": "0.002418", "module": "C3", "scenario": "S1"}, {"value": "0.0002176", "module": "C3", "scenario": "S2"}, {"value": "0", "module": "C4"}, {"value": "-0.007165", "module": "D", "scenario": "S1"}, {"value": "-0.00154", "module": "D", "scenario": "S2"}]}}, {"referenceToLCIAMethodDataSet": {"shortDescription": [{"value": "Potenzial für den abiotischen Abbau nicht fossiler Ressourcen (ADPE)", "lang": "de"}, {"value": "Abiotic depletion potential for non fossil resources (ADPE)", "lang": "en"}], "type": "LCIA method data set", "refObjectId": "b2ad6494-c78d-11e6-9d9d-cec0c932ce01", "uri": "../lciamethods/b2ad6494-c78d-11e6-9d9d-cec0c932ce01.xml"}, "other": {"anies": [{"name": "referenceToUnitGroupDataSet", "value": {"shortDescription": [{"value": "kg Sb-Äq.", "lang": "de"}], "type": "unit group data set", "refObjectId": "54ccd2d9-a32a-4fc2-923d-f2c8c93e89d4", "uri": "../unitgroups/54ccd2d9-a32a-4fc2-923d-f2c8c93e89d4.xml"}}, {"value": "9.061E-06", "module": "A1-A3"}, {"value": "1.175E-09", "module": "A5"}, {"value": "1.503E-06", "module": "B2"}, {"value": "1.296E-07", "module": "B5"}, {"value": "0", "module": "C1"}, {"value": "1.086E-08", "module": "C2"}, {"value": "3.808E-08", "module": "C3", "scenario": "S1"}, {"value": "3.55E-07", "module": "C3", "scenario": "S2"}, {"value": "0", "module": "C4"}, {"value": "-1.144E-06", "module": "D", "scenario": "S1"}, {"value": "-3.263E-06", "module": "D", "scenario": "S2"}]}}, {"referenceToLCIAMethodDataSet": {"shortDescription": [{"value": "Potenzial für den abiotischen Abbau fossiler Brennstoffe (ADPF)", "lang": "de"}, {"value": "Abiotic depletion potential for fossil resources (ADPF)", "lang": "en"}], "type": "LCIA method data set", "refObjectId": "b2ad6110-c78d-11e6-9d9d-cec0c932ce01", "uri": "../lciamethods/b2ad6110-c78d-11e6-9d9d-cec0c932ce01.xml"}, "other": {"anies": [{"name": "referenceToUnitGroupDataSet", "value": {"shortDescription": [{"value": "MJ", "lang": "de"}], "type": "unit group data set", "refObjectId": "93a60a57-a3c8-11da-a746-0800200c9a66", "uri": "../unitgroups/93a60a57-a3c8-11da-a746-0800200c9a66.xml"}}, {"value": "178.4", "module": "A1-A3"}, {"value": "0.1399", "module": "A5"}, {"value": "97.64", "module": "B2"}, {"value": "15.47", "module": "B5"}, {"value": "0", "module": "C1"}, {"value": "1.632", "module": "C2"}, {"value": "4.144", "module": "C3", "scenario": "S1"}, {"value": "2.125", "module": "C3", "scenario": "S2"}, {"value": "0", "module": "C4"}, {"value": "-119.1", "module": "D", "scenario": "S1"}, {"value": "-5.065", "module": "D", "scenario": "S2"}]}}, {"referenceToLCIAMethodDataSet": {"shortDescription": [{"value": "Wassernutzung (WDP)", "lang": "de"}, {"value": "Water use (WDP)", "lang": "en"}], "type": "LCIA method data set", "refObjectId": "b2ad66ce-c78d-11e6-9d9d-cec0c932ce01", "uri": "../lciamethods/b2ad66ce-c78d-11e6-9d9d-cec0c932ce01.xml"}, "other": {"anies": [{"name": "referenceToUnitGroupDataSet", "value": {"shortDescription": [{"value": "m^(3) Welt-Äq. entzogen", "lang": "de"}], "type": "unit group data set", "refObjectId": "6ae2df01-888e-46c8-b17d-49fa3869b476", "uri": "../unitgroups/6ae2df01-888e-46c8-b17d-49fa3869b476.xml"}}, {"value": "1.009", "module": "A1-A3"}, {"value": "0.04869", "module": "A5"}, {"value": "0.8787", "module": "B2"}, {"value": "0.2336", "module": "B5"}, {"value": "0", "module": "C1"}, {"value": "0.001137", "module": "C2"}, {"value": "1.971", "module": "C3", "scenario": "S1"}, {"value": "0.06695", "module": "C3", "scenario": "S2"}, {"value": "0", "module": "C4"}, {"value": "-0.5281", "module": "D", "scenario": "S1"}, {"value": "-0.08403", "module": "D", "scenario": "S2"}]}}, {"referenceToLCIAMethodDataSet": {"shortDescription": [{"value": "Auftreten von Krankheiten aufgrund von Feinstaubemissionen (PM)", "lang": "de"}, {"value": "Incidence of disease due to PM emissions (PM)", "lang": "en"}], "type": "LCIA method data set", "refObjectId": "b5c602c6-def3-11e6-bf01-fe55135034f3", "uri": "../lciamethods/b5c602c6-def3-11e6-bf01-fe55135034f3.xml"}, "other": {"anies": [{"name": "referenceToUnitGroupDataSet", "value": {"shortDescription": [{"value": "Krankheitsfälle", "lang": "de"}], "type": "unit group data set", "refObjectId": "3883559b-648f-4afc-8ba2-0bd24f3affa3", "uri": "../unitgroups/3883559b-648f-4afc-8ba2-0bd24f3affa3.xml"}}, {"module": "A1-A3"}, {"module": "A5"}, {"module": "B2"}, {"module": "B5"}, {"module": "C1"}, {"module": "C2"}, {"module": "C3", "scenario": "S1"}, {"module": "C3", "scenario": "S2"}, {"module": "C4"}, {"module": "D", "scenario": "S1"}, {"module": "D", "scenario": "S2"}]}}, {"referenceToLCIAMethodDataSet": {"shortDescription": [{"value": "Wirkung durch Exposition des Menschen mit U235 (IR)", "lang": "de"}, {"value": "Human exposure efficiency relative to U235 (IR)", "lang": "en"}], "type": "LCIA method data set", "refObjectId": "b5c632be-def3-11e6-bf01-fe55135034f3", "uri": "../lciamethods/b5c632be-def3-11e6-bf01-fe55135034f3.xml"}, "other": {"anies": [{"name": "referenceToUnitGroupDataSet", "value": {"shortDescription": [{"value": "kBq U235-Äq.", "lang": "de"}], "type": "unit group data set", "refObjectId": "456b05bf-1415-44a9-9993-02452f554c09", "uri": "../unitgroups/456b05bf-1415-44a9-9993-02452f554c09.xml"}}, {"module": "A1-A3"}, {"module": "A5"}, {"module": "B2"}, {"module": "B5"}, {"module": "C1"}, {"module": "C2"}, {"module": "C3", "scenario": "S1"}, {"module": "C3", "scenario": "S2"}, {"module": "C4"}, {"module": "D", "scenario": "S1"}, {"module": "D", "scenario": "S2"}]}}, {"referenceToLCIAMethodDataSet": {"shortDescription": [{"value": "Toxizitätsvergleichseinheit für Ökosysteme (ETP-fw)", "lang": "de"}, {"value": "Comparative toxic unit for ecosystems (ETP-fw)", "lang": "en"}], "type": "LCIA method data set", "refObjectId": "ee1082d1-b0f7-43ca-a1f0-21e2a4a74511", "uri": "../lciamethods/ee1082d1-b0f7-43ca-a1f0-21e2a4a74511.xml"}, "other": {"anies": [{"name": "referenceToUnitGroupDataSet", "value": {"shortDescription": [{"value": "CTUe", "lang": "de"}], "type": "unit group data set", "refObjectId": "aa959ded-f1eb-4efb-9c5c-2d60be36b3e6", "uri": "../unitgroups/aa959ded-f1eb-4efb-9c5c-2d60be36b3e6.xml"}}, {"module": "A1-A3"}, {"module": "A5"}, {"module": "B2"}, {"module": "B5"}, {"module": "C1"}, {"module": "C2"}, {"module": "C3", "scenario": "S1"}, {"module": "C3", "scenario": "S2"}, {"module": "C4"}, {"module": "D", "scenario": "S1"}, {"module": "D", "scenario": "S2"}]}}, {"referenceToLCIAMethodDataSet": {"shortDescription": [{"value": "Toxizitätsvergleichseinheit für Menschen (krebserregend) (HTP-c)", "lang": "de"}, {"value": "Comparative toxic unit for humans (carcinogenic) (HTP-c)", "lang": "en"}], "type": "LCIA method data set", "refObjectId": "2299222a-bbd8-474f-9d4f-4dd1f18aea7c", "uri": "../lciamethods/2299222a-bbd8-474f-9d4f-4dd1f18aea7c.xml"}, "other": {"anies": [{"name": "referenceToUnitGroupDataSet", "value": {"shortDescription": [{"value": "CTUh", "lang": "de"}], "type": "unit group data set", "refObjectId": "d4c9523e-2d7e-49fd-8469-998f547d3a70", "uri": "../unitgroups/d4c9523e-2d7e-49fd-8469-998f547d3a70.xml"}}, {"module": "A1-A3"}, {"module": "A5"}, {"module": "B2"}, {"module": "B5"}, {"module": "C1"}, {"module": "C2"}, {"module": "C3", "scenario": "S1"}, {"module": "C3", "scenario": "S2"}, {"module": "C4"}, {"module": "D", "scenario": "S1"}, {"module": "D", "scenario": "S2"}]}}, {"referenceToLCIAMethodDataSet": {"shortDescription": [{"value": "Toxizitätsvergleichseinheit für Menschen (nicht krebserregend) (HTP-nc)", "lang": "de"}, {"value": "Comparative toxic unit for humans (noncarcinogenic) (HTP-nc)", "lang": "en"}], "type": "LCIA method data set", "refObjectId": "3af763a5-b7a1-48c9-9cee-1f223481fcef", "uri": "../lciamethods/3af763a5-b7a1-48c9-9cee-1f223481fcef.xml"}, "other": {"anies": [{"name": "referenceToUnitGroupDataSet", "value": {"shortDescription": [{"value": "CTUh", "lang": "de"}], "type": "unit group data set", "refObjectId": "d4c9523e-2d7e-49fd-8469-998f547d3a70", "uri": "../unitgroups/d4c9523e-2d7e-49fd-8469-998f547d3a70.xml"}}, {"module": "A1-A3"}, {"module": "A5"}, {"module": "B2"}, {"module": "B5"}, {"module": "C1"}, {"module": "C2"}, {"module": "C3", "scenario": "S1"}, {"module": "C3", "scenario": "S2"}, {"module": "C4"}, {"module": "D", "scenario": "S1"}, {"module": "D", "scenario": "S2"}]}}, {"referenceToLCIAMethodDataSet": {"shortDescription": [{"value": "Bodenqualitätsindex (SQP)", "lang": "de"}, {"value": "Soil quality index (SQP)", "lang": "en"}], "type": "LCIA method data set", "refObjectId": "b2ad6890-c78d-11e6-9d9d-cec0c932ce01", "uri": "../lciamethods/b2ad6890-c78d-11e6-9d9d-cec0c932ce01.xml"}, "other": {"anies": [{"name": "referenceToUnitGroupDataSet", "value": {"shortDescription": [{"value": "SQP", "lang": "de"}], "type": "unit group data set", "refObjectId": "f130951c-e67f-4f7f-8dd4-665de3974e18", "uri": "../unitgroups/f130951c-e67f-4f7f-8dd4-665de3974e18.xml"}}, {"module": "A1-A3"}, {"module": "A5"}, {"module": "B2"}, {"module": "B5"}, {"module": "C1"}, {"module": "C2"}, {"module": "C3", "scenario": "S1"}, {"module": "C3", "scenario": "S2"}, {"module": "C4"}, {"module": "D", "scenario": "S1"}, {"module": "D", "scenario": "S2"}]}}]}, "otherAttributes": {"{http://www.indata.network/EPD/2019}epd-version": "1.2"}, "version": "1.1", "locations": "../ILCDLocations.xml"}