{"processInformation": {"dataSetInformation": {"UUID": "a213836d-1a3f-4bf7-8d60-8dc7899e069d", "name": {"baseName": [{"value": "StoSilent Board 100 S; 105 C; 110 S", "lang": "en"}]}, "classificationInformation": {"classification": [{"class": [{"value": "Dämmstoffe", "level": 0, "classId": "2"}, {"value": "Schaumglas", "level": 1, "classId": "2.6"}, {"value": "Platten", "level": 2, "classId": "2.6.01"}], "name": "OEKOBAU.DAT"}]}, "generalComment": [{"value": "The owner of this EPD shall be liable for the underlying information and evidence. The programme operator Kiwa-Ecobility Experts shall not be liable with respect to manufacturer data, life cycle assessment data and evidence.", "lang": "en"}], "other": {"anies": [{"scenario": [{"description": [{"value": "1% cut off criteria have been applied for formulation and production data when applicable according to DIN EN 15804+A2. No machines are needed for the product at the deconstruction / demolition phase."}], "name": "Standard scenario", "default": true}]}, "<ns11:modules xmlns:ns11=\"http://openlca.org/epd_ilcd\" xmlns=\"http://lca.jrc.it/ILCD/Process\" xmlns:c=\"http://lca.jrc.it/ILCD/Contact\" xmlns:common=\"http://lca.jrc.it/ILCD/Common\" xmlns:epd=\"http://www.iai.kit.edu/EPD/2013\" xmlns:epd2=\"http://www.indata.network/EPD/2019\" xmlns:f=\"http://lca.jrc.it/ILCD/Flow\" xmlns:fp=\"http://lca.jrc.it/ILCD/FlowProperty\" xmlns:m=\"http://lca.jrc.it/ILCD/LCIAMethod\" xmlns:ns9=\"http://www.okworx.com/ILCD/Extensions/2018/Profile\" xmlns:s=\"http://lca.jrc.it/ILCD/Source\" xmlns:u=\"http://lca.jrc.it/ILCD/UnitGroup\" name=\"A1\" scenario=\"Standard scenario\"/>", "<ns11:modules xmlns:ns11=\"http://openlca.org/epd_ilcd\" xmlns=\"http://lca.jrc.it/ILCD/Process\" xmlns:c=\"http://lca.jrc.it/ILCD/Contact\" xmlns:common=\"http://lca.jrc.it/ILCD/Common\" xmlns:epd=\"http://www.iai.kit.edu/EPD/2013\" xmlns:epd2=\"http://www.indata.network/EPD/2019\" xmlns:f=\"http://lca.jrc.it/ILCD/Flow\" xmlns:fp=\"http://lca.jrc.it/ILCD/FlowProperty\" xmlns:m=\"http://lca.jrc.it/ILCD/LCIAMethod\" xmlns:ns9=\"http://www.okworx.com/ILCD/Extensions/2018/Profile\" xmlns:s=\"http://lca.jrc.it/ILCD/Source\" xmlns:u=\"http://lca.jrc.it/ILCD/UnitGroup\" name=\"A2\" scenario=\"Standard scenario\"/>", "<ns11:modules xmlns:ns11=\"http://openlca.org/epd_ilcd\" xmlns=\"http://lca.jrc.it/ILCD/Process\" xmlns:c=\"http://lca.jrc.it/ILCD/Contact\" xmlns:common=\"http://lca.jrc.it/ILCD/Common\" xmlns:epd=\"http://www.iai.kit.edu/EPD/2013\" xmlns:epd2=\"http://www.indata.network/EPD/2019\" xmlns:f=\"http://lca.jrc.it/ILCD/Flow\" xmlns:fp=\"http://lca.jrc.it/ILCD/FlowProperty\" xmlns:m=\"http://lca.jrc.it/ILCD/LCIAMethod\" xmlns:ns9=\"http://www.okworx.com/ILCD/Extensions/2018/Profile\" xmlns:s=\"http://lca.jrc.it/ILCD/Source\" xmlns:u=\"http://lca.jrc.it/ILCD/UnitGroup\" name=\"A3\" scenario=\"Standard scenario\"/>", "<ns11:modules xmlns:ns11=\"http://openlca.org/epd_ilcd\" xmlns=\"http://lca.jrc.it/ILCD/Process\" xmlns:c=\"http://lca.jrc.it/ILCD/Contact\" xmlns:common=\"http://lca.jrc.it/ILCD/Common\" xmlns:epd=\"http://www.iai.kit.edu/EPD/2013\" xmlns:epd2=\"http://www.indata.network/EPD/2019\" xmlns:f=\"http://lca.jrc.it/ILCD/Flow\" xmlns:fp=\"http://lca.jrc.it/ILCD/FlowProperty\" xmlns:m=\"http://lca.jrc.it/ILCD/LCIAMethod\" xmlns:ns9=\"http://www.okworx.com/ILCD/Extensions/2018/Profile\" xmlns:s=\"http://lca.jrc.it/ILCD/Source\" xmlns:u=\"http://lca.jrc.it/ILCD/UnitGroup\" name=\"A4\" scenario=\"Standard scenario\"/>", "<ns11:modules xmlns:ns11=\"http://openlca.org/epd_ilcd\" xmlns=\"http://lca.jrc.it/ILCD/Process\" xmlns:c=\"http://lca.jrc.it/ILCD/Contact\" xmlns:common=\"http://lca.jrc.it/ILCD/Common\" xmlns:epd=\"http://www.iai.kit.edu/EPD/2013\" xmlns:epd2=\"http://www.indata.network/EPD/2019\" xmlns:f=\"http://lca.jrc.it/ILCD/Flow\" xmlns:fp=\"http://lca.jrc.it/ILCD/FlowProperty\" xmlns:m=\"http://lca.jrc.it/ILCD/LCIAMethod\" xmlns:ns9=\"http://www.okworx.com/ILCD/Extensions/2018/Profile\" xmlns:s=\"http://lca.jrc.it/ILCD/Source\" xmlns:u=\"http://lca.jrc.it/ILCD/UnitGroup\" name=\"A5\" scenario=\"Standard scenario\"/>", "<ns11:modules xmlns:ns11=\"http://openlca.org/epd_ilcd\" xmlns=\"http://lca.jrc.it/ILCD/Process\" xmlns:c=\"http://lca.jrc.it/ILCD/Contact\" xmlns:common=\"http://lca.jrc.it/ILCD/Common\" xmlns:epd=\"http://www.iai.kit.edu/EPD/2013\" xmlns:epd2=\"http://www.indata.network/EPD/2019\" xmlns:f=\"http://lca.jrc.it/ILCD/Flow\" xmlns:fp=\"http://lca.jrc.it/ILCD/FlowProperty\" xmlns:m=\"http://lca.jrc.it/ILCD/LCIAMethod\" xmlns:ns9=\"http://www.okworx.com/ILCD/Extensions/2018/Profile\" xmlns:s=\"http://lca.jrc.it/ILCD/Source\" xmlns:u=\"http://lca.jrc.it/ILCD/UnitGroup\" name=\"C1\" scenario=\"Standard scenario\"/>", "<ns11:modules xmlns:ns11=\"http://openlca.org/epd_ilcd\" xmlns=\"http://lca.jrc.it/ILCD/Process\" xmlns:c=\"http://lca.jrc.it/ILCD/Contact\" xmlns:common=\"http://lca.jrc.it/ILCD/Common\" xmlns:epd=\"http://www.iai.kit.edu/EPD/2013\" xmlns:epd2=\"http://www.indata.network/EPD/2019\" xmlns:f=\"http://lca.jrc.it/ILCD/Flow\" xmlns:fp=\"http://lca.jrc.it/ILCD/FlowProperty\" xmlns:m=\"http://lca.jrc.it/ILCD/LCIAMethod\" xmlns:ns9=\"http://www.okworx.com/ILCD/Extensions/2018/Profile\" xmlns:s=\"http://lca.jrc.it/ILCD/Source\" xmlns:u=\"http://lca.jrc.it/ILCD/UnitGroup\" name=\"C2\" scenario=\"Standard scenario\"/>", "<ns11:modules xmlns:ns11=\"http://openlca.org/epd_ilcd\" xmlns=\"http://lca.jrc.it/ILCD/Process\" xmlns:c=\"http://lca.jrc.it/ILCD/Contact\" xmlns:common=\"http://lca.jrc.it/ILCD/Common\" xmlns:epd=\"http://www.iai.kit.edu/EPD/2013\" xmlns:epd2=\"http://www.indata.network/EPD/2019\" xmlns:f=\"http://lca.jrc.it/ILCD/Flow\" xmlns:fp=\"http://lca.jrc.it/ILCD/FlowProperty\" xmlns:m=\"http://lca.jrc.it/ILCD/LCIAMethod\" xmlns:ns9=\"http://www.okworx.com/ILCD/Extensions/2018/Profile\" xmlns:s=\"http://lca.jrc.it/ILCD/Source\" xmlns:u=\"http://lca.jrc.it/ILCD/UnitGroup\" name=\"C3\" scenario=\"Standard scenario\"/>", "<ns11:modules xmlns:ns11=\"http://openlca.org/epd_ilcd\" xmlns=\"http://lca.jrc.it/ILCD/Process\" xmlns:c=\"http://lca.jrc.it/ILCD/Contact\" xmlns:common=\"http://lca.jrc.it/ILCD/Common\" xmlns:epd=\"http://www.iai.kit.edu/EPD/2013\" xmlns:epd2=\"http://www.indata.network/EPD/2019\" xmlns:f=\"http://lca.jrc.it/ILCD/Flow\" xmlns:fp=\"http://lca.jrc.it/ILCD/FlowProperty\" xmlns:m=\"http://lca.jrc.it/ILCD/LCIAMethod\" xmlns:ns9=\"http://www.okworx.com/ILCD/Extensions/2018/Profile\" xmlns:s=\"http://lca.jrc.it/ILCD/Source\" xmlns:u=\"http://lca.jrc.it/ILCD/UnitGroup\" name=\"C4\" scenario=\"Standard scenario\"/>", "<ns11:modules xmlns:ns11=\"http://openlca.org/epd_ilcd\" xmlns=\"http://lca.jrc.it/ILCD/Process\" xmlns:c=\"http://lca.jrc.it/ILCD/Contact\" xmlns:common=\"http://lca.jrc.it/ILCD/Common\" xmlns:epd=\"http://www.iai.kit.edu/EPD/2013\" xmlns:epd2=\"http://www.indata.network/EPD/2019\" xmlns:f=\"http://lca.jrc.it/ILCD/Flow\" xmlns:fp=\"http://lca.jrc.it/ILCD/FlowProperty\" xmlns:m=\"http://lca.jrc.it/ILCD/LCIAMethod\" xmlns:ns9=\"http://www.okworx.com/ILCD/Extensions/2018/Profile\" xmlns:s=\"http://lca.jrc.it/ILCD/Source\" xmlns:u=\"http://lca.jrc.it/ILCD/UnitGroup\" name=\"D\" scenario=\"Standard scenario\"/>"]}}, "quantitativeReference": {"referenceToReferenceFlow": [1], "type": "Reference flow(s)"}, "time": {"referenceYear": 2023, "dataSetValidUntil": 2029, "timeRepresentativenessDescription": [{"value": "Formulation and production information based on year 2023\r.", "lang": "en"}], "other": {"anies": [{"name": "publicationDateOfEPD", "value": 1718668800000}]}}, "geography": {"locationOfOperationSupplyOrProduction": {"descriptionOfRestrictions": [{"value": "The data is representative for the European Union.", "lang": "en"}], "location": "EU-27"}}, "technology": {"technologyDescriptionAndIncludedProcesses": [{"value": "This EPD is representative for StoSilent Board 100 S, StoSilent Board 105 C and StoSilent Board 110 S. The input data used is based on StoSilent Board 110 S which demonstrates the highest environmental impact of the group due to its mass per m2.  Acoustic panel made of expanded glass granulate for suspended ceiling and wall structures. Area of application: interior, for suspended ceiling and wall structures. The boards, StoSilent Board 100 S and 105 C and 110 S, are manufactured at production sites in Ilmenau and Lauingen. In Ilmenau, all raw materials are getting mixed, formed into shape, dried, tempered, cut and sanded to format, packaged on pallets and forwarded to Lauingen for further processing. At Lauingen, lamination of non-woven fleece on front and rear under pressure, cut to format, application of edge coating and packaging.", "lang": "en"}], "technologicalApplicability": [{"value": "For suspended ceiling and wall coverings on level surfaces, Rooms with high visual standards, for balanced acoustics and good noise reduction. Application: StoSilent Board 105 C:  adhesive fixed; StoSilent Board 110 S: screw fixed, bonded board joints; StoSilent Board 100 S: screw fixed, bonded board joints. Area of application: Building interiors; In buildings designed for people to reside in; In buildings with the usual interior climatic conditions; Examples: high-quality offices, living spaces, hotel rooms. Properties: up to 200 m² possible without expansion joint (max. side length: 20 m); reduction in the reverberation time; reduction of noise level; improved ability to concentrate; improvement in speech intelligibility; low weight; high degree of stiffness; low moisture-induced and thermal expansion. Format: board edge: sharp-edged/coated; length x width x thickness: 1200 x 625 x 25 mm.", "lang": "en"}], "referenceToTechnologyFlowDiagrammOrPicture": [{"shortDescription": [{"value": "Flow chart StoSilent Board 100 S; 105 C; 110 S", "lang": "en"}], "type": "source data set", "refObjectId": "3bd64192-540a-431c-a6a3-0a80e65a1156", "version": "00.00.001"}]}}, "modellingAndValidation": {"LCIMethodAndAllocation": {"typeOfDataSet": "EPD", "other": {"anies": [{"name": "subType", "value": "specific dataset"}]}}, "dataSourcesTreatmentAndRepresentativeness": {"referenceToDataSource": [{"shortDescription": [{"value": "ecoinvent 3.6 database", "lang": "en"}], "type": "source data set", "refObjectId": "766b9973-5ee8-48a2-8098-72c8e20b369f", "version": "00.00.001"}, {"shortDescription": [{"value": "ecoinvent database (general)", "lang": "en"}], "type": "source data set", "refObjectId": "b497a91f-e14b-4b69-8f28-f50eb1576766", "version": "00.03.002"}], "useAdviceForDataSet": [{"value": "For suspended ceiling and wall coverings on level surfaces, Rooms with high visual standards, for balanced acoustics and good noise reduction. Application: StoSilent Board 105 C:  adhesive fixed; StoSilent Board 110 S: screw fixed, bonded board joints; StoSilent Board 100 S: screw fixed, bonded board joints. Area of application: Building interiors; In buildings designed for people to reside in; In buildings with the usual interior climatic conditions; Examples: high-quality offices, living spaces, hotel rooms. Properties: up to 200 m² possible without expansion joint (max. side length: 20 m); reduction in the reverberation time; reduction of noise level; improved ability to concentrate; improvement in speech intelligibility; low weight; high degree of stiffness; low moisture-induced and thermal expansion. Format: board edge: sharp-edged/coated; length x width x thickness: 1200 x 625 x 25 mm.", "lang": "en"}], "other": {"anies": [{"name": "referenceToOriginalEPD", "value": {"shortDescription": {"value": "StoSilent Board 100 S; 105 C; 110 S EPD", "defaultValue": "StoSilent Board 100 S; 105 C; 110 S EPD", "lstrings": [{"lang": "en", "value": "StoSilent Board 100 S; 105 C; 110 S EPD"}]}, "version": {"version": 3, "majorVersion": 0, "minorVersion": 0, "subMinorVersion": 3, "zero": false, "versionString": "00.00.003"}, "type": "source data set", "uuid": {"uuid": "8e22fcce-b2c0-461a-8919-ee3364820b10"}, "refObjectId": "8e22fcce-b2c0-461a-8919-ee3364820b10", "versionAsString": "00.00.003", "resourceURLs": ["https://oekobaudat.de/OEKOBAU.DAT/resource/sources/8e22fcce-b2c0-461a-8919-ee3364820b10/EPD-Kiwa-EE-140610-EN.pdf?version=00.00.003"]}}]}}, "validation": {"review": [{"reviewDetails": [{"value": "The independent verification is in accordance with the ISO 14025:2011.", "lang": "en"}], "referenceToNameOfReviewerAndInstitution": [{"shortDescription": [{"value": "Lucas Pedro Berman, Senda", "lang": "en"}], "type": "contact data set", "refObjectId": "2294137c-5a52-4a75-965f-770e74b24b10", "version": "00.00.002"}], "type": "Independent external review"}]}, "complianceDeclarations": {"compliance": [{"referenceToComplianceSystem": {"shortDescription": [{"value": "ISO 14025", "lang": "en"}], "type": "source data set", "refObjectId": "4f2eb655-6e44-4874-a95a-e28f5442cd4d", "version": "00.00.001"}}, {"referenceToComplianceSystem": {"shortDescription": [{"value": "EN 15804+A2 (EF 3.0)", "lang": "de"}, {"value": "EN 15804+A2 (EF 3.0)", "lang": "en"}], "type": "source data set", "refObjectId": "c0016b33-8cf7-415c-ac6e-deba0d21440d", "version": "00.02.000"}}]}}, "administrativeInformation": {"commissionerAndGoal": {"referenceToCommissioner": [{"shortDescription": [{"value": "Sto SE & Co. KGaA", "lang": "en"}], "type": "contact data set", "refObjectId": "cac5aef9-26f0-4d83-beb8-d9f54cb53669", "version": "00.00.001"}]}, "dataGenerator": {"referenceToPersonOrEntityGeneratingTheDataSet": [{"shortDescription": [{"value": "Sto Scandinavia AB", "lang": "en"}], "type": "contact data set", "refObjectId": "e7fe9f30-f7fc-4fe4-95b6-f0240a4c6199", "version": "00.00.001"}]}, "dataEntryBy": {"timeStamp": 1752225638897, "referenceToDataSetFormat": [{"shortDescription": [{"value": "EPD Data Format Extensions v1.2", "lang": "en"}, {"value": "EPD-Datenformaterweiterungen v1.2", "lang": "de"}], "type": "source data set", "refObjectId": "a29449fd-aa2f-4de8-b5d7-4b06b43c6fde", "version": "00.01.000"}, {"shortDescription": [{"value": "ILCD format", "lang": "en"}], "type": "source data set", "refObjectId": "a97a0155-0234-4b87-b4ce-a45da52f2a40", "version": "01.00.001", "uri": "http://lca.jrc.ec.europa.eu/lcainfohub/sample_data/ilcd/sources/ILCD_Format_a97a0155-0234-4b87-b4ce-a45da52f2a40_01.00.000.xml"}], "referenceToPersonOrEntityEnteringTheData": {"shortDescription": [{"value": "Kiwa GmbH (Berlin)", "lang": "en"}], "type": "contact data set", "refObjectId": "3ea4a87a-3f88-4633-b7e7-1bbdd272be43", "version": "00.00.002"}}, "publicationAndOwnership": {"dataSetVersion": "00.00.020", "referenceToRegistrationAuthority": {"shortDescription": [{"value": "Kiwa-Ecobility Experts, Kiwa GmbH (Berlin)", "lang": "en"}], "type": "contact data set", "refObjectId": "eb52a9a8-9d0f-40ce-a5c9-7b78f5615e5a", "version": "00.00.002"}, "registrationNumber": "EPD-Kiwa-EE-140610-EN", "referenceToOwnershipOfDataSet": {"shortDescription": [{"value": "Sto SE & Co. KGaA", "lang": "en"}], "type": "contact data set", "refObjectId": "cac5aef9-26f0-4d83-beb8-d9f54cb53669", "version": "00.00.001"}, "copyright": true, "licenseType": "Free of charge for all users and uses", "accessRestrictions": [{"value": "None.", "lang": "en"}], "other": {"anies": [{"name": "referenceToPublisher", "value": {"shortDescription": [{"value": "Kiwa-Ecobility Experts, Kiwa GmbH (Berlin)", "lang": "en"}], "type": "contact data set", "refObjectId": "eb52a9a8-9d0f-40ce-a5c9-7b78f5615e5a", "version": "00.00.002"}}]}}}, "exchanges": {"exchange": [{"dataSetInternalID": 1, "referenceToFlowDataSet": {"shortDescription": [{"value": "StoSilent Board 100 S; 105 C; 110 S", "lang": "en"}], "type": "flow data set", "refObjectId": "fbf14beb-99f2-4141-a31a-572b110cc9eb", "version": "00.00.004"}, "meanAmount": 1.0, "resultingAmount": 1.0, "referenceFlow": true, "resultingflowAmount": 1.0, "flowProperties": [{"name": [{"lang": "de", "value": "Fläche"}, {"lang": "en", "value": "Area"}], "uuid": "93a60a56-a3c8-19da-a746-0800200c9a66", "referenceFlowProperty": true, "meanValue": 1.0, "referenceUnit": "qm", "unitGroupUUID": "c20a03d7-bd90-4569-bc94-66cfd364dfc8"}], "materialProperties": [{"name": "grammage", "value": "6.938", "unit": "kg/m^2", "unitDescription": "kilograms per square meter"}, {"name": "layer thickness", "value": "0.025", "unit": "m", "unitDescription": "meters"}], "typeOfFlow": "Product flow", "classification": {"classHierarchy": "Dämmstoffe / Schaumglas / Platten", "name": "OEKOBAU.DAT"}}, {"dataSetInternalID": 2, "referenceToFlowDataSet": {"shortDescription": [{"value": "Komponenten für die Wiederverwendung (CRU)", "lang": "de"}, {"value": "Components for re-use (CRU)", "lang": "en"}, {"value": "Componentes para su reutilización (CRU)", "lang": "es"}, {"value": "Komponenter för återanvändning (CRU)", "lang": "sv"}], "type": "flow data set", "refObjectId": "a2b32f97-3fc7-4af2-b209-525bc6426f33", "version": "30.00.002"}, "exchange direction": "OUTPUT", "meanAmount": 0.0, "other": {"anies": [{"value": "0.0", "module": "A1", "scenario": "Standard scenario"}, {"value": "0.0", "module": "A2", "scenario": "Standard scenario"}, {"value": "0.0", "module": "A3", "scenario": "Standard scenario"}, {"value": "0.0", "module": "A4", "scenario": "Standard scenario"}, {"value": "0.0096", "module": "A5", "scenario": "Standard scenario"}, {"value": "0.0", "module": "C1", "scenario": "Standard scenario"}, {"value": "0.0", "module": "C2", "scenario": "Standard scenario"}, {"value": "0.0", "module": "C3", "scenario": "Standard scenario"}, {"value": "0.0", "module": "C4", "scenario": "Standard scenario"}, {"value": "0.0", "module": "D", "scenario": "Standard scenario"}, {"name": "referenceToUnitGroupDataSet", "value": {"shortDescription": [{"value": "kg"}], "type": "unit group data set", "refObjectId": "ad38d542-3fe9-439d-9b95-2f5f7752acaf", "uri": "../unitgroups/ad38d542-3fe9-439d-9b95-2f5f7752acaf"}}]}, "resolvedFlowVersion": "38.00.000", "flowProperties": [], "typeOfFlow": "Other flow", "classification": {"classHierarchy": "Quantities / Environmental quantities / EPD EN 15804 / LCI indicators", "name": "GaBiCategories"}}, {"dataSetInternalID": 3, "referenceToFlowDataSet": {"shortDescription": [{"value": "Exportierte elektrische Energie (EEE)", "lang": "de"}, {"value": "Exported electrical energy (EEE)", "lang": "en"}, {"value": "Energía exportada electrica (EEE)", "lang": "es"}, {"value": "Exporterad energi – elektrisk (EEE)", "lang": "sv"}], "type": "flow data set", "refObjectId": "4da0c987-2b76-40d6-9e9e-82a017aaaf29", "version": "30.00.002"}, "exchange direction": "OUTPUT", "meanAmount": 0.0, "other": {"anies": [{"value": "0.0", "module": "A1", "scenario": "Standard scenario"}, {"value": "0.0", "module": "A2", "scenario": "Standard scenario"}, {"value": "0.0", "module": "A3", "scenario": "Standard scenario"}, {"value": "0.0", "module": "A4", "scenario": "Standard scenario"}, {"value": "0.0", "module": "A5", "scenario": "Standard scenario"}, {"value": "0.0", "module": "C1", "scenario": "Standard scenario"}, {"value": "0.0", "module": "C2", "scenario": "Standard scenario"}, {"value": "0.0", "module": "C3", "scenario": "Standard scenario"}, {"value": "0.0", "module": "C4", "scenario": "Standard scenario"}, {"value": "2.4863041044", "module": "D", "scenario": "Standard scenario"}, {"name": "referenceToUnitGroupDataSet", "value": {"shortDescription": [{"value": "MJ"}], "type": "unit group data set", "refObjectId": "93a60a57-a3c8-11da-a746-0800200c9a66", "uri": "../unitgroups/93a60a57-a3c8-11da-a746-0800200c9a66"}}]}, "resolvedFlowVersion": "38.00.000", "flowProperties": [], "typeOfFlow": "Other flow", "classification": {"classHierarchy": "Quantities / Environmental quantities / EPD EN 15804 / LCI indicators", "name": "GaBiCategories"}}, {"dataSetInternalID": 4, "referenceToFlowDataSet": {"shortDescription": [{"value": "Exportierte thermische Energie (EET)", "lang": "de"}, {"value": "Exported thermal energy (EET)", "lang": "en"}, {"value": "Energía exportada termal (EET)", "lang": "es"}, {"value": "Exporterad energi – termisk (EET)", "lang": "sv"}], "type": "flow data set", "refObjectId": "98daf38a-7a79-46d3-9a37-2b7bd0955810", "version": "30.00.002"}, "exchange direction": "OUTPUT", "meanAmount": 0.0, "other": {"anies": [{"value": "0.0", "module": "A1", "scenario": "Standard scenario"}, {"value": "0.0", "module": "A2", "scenario": "Standard scenario"}, {"value": "0.0", "module": "A3", "scenario": "Standard scenario"}, {"value": "0.0", "module": "A4", "scenario": "Standard scenario"}, {"value": "0.0", "module": "A5", "scenario": "Standard scenario"}, {"value": "0.0", "module": "C1", "scenario": "Standard scenario"}, {"value": "0.0", "module": "C2", "scenario": "Standard scenario"}, {"value": "0.0", "module": "C3", "scenario": "Standard scenario"}, {"value": "0.0", "module": "C4", "scenario": "Standard scenario"}, {"value": "4.2819681798", "module": "D", "scenario": "Standard scenario"}, {"name": "referenceToUnitGroupDataSet", "value": {"shortDescription": [{"value": "MJ"}], "type": "unit group data set", "refObjectId": "93a60a57-a3c8-11da-a746-0800200c9a66", "uri": "../unitgroups/93a60a57-a3c8-11da-a746-0800200c9a66"}}]}, "resolvedFlowVersion": "38.00.000", "flowProperties": [], "typeOfFlow": "Other flow", "classification": {"classHierarchy": "Quantities / Environmental quantities / EPD EN 15804 / LCI indicators", "name": "GaBiCategories"}}, {"dataSetInternalID": 5, "referenceToFlowDataSet": {"shortDescription": [{"value": "Gefährlicher Abfall zur Deponie (HWD)", "lang": "de"}, {"value": "Hazardous waste disposed (HWD)", "lang": "en"}, {"value": "Residuos peligrosos eliminados (HWD)", "lang": "es"}, {"value": "Farligt avfall (HWD)", "lang": "sv"}], "type": "flow data set", "refObjectId": "430f9e0f-59b2-46a0-8e0d-55e0e84948fc", "version": "30.00.002"}, "exchange direction": "OUTPUT", "meanAmount": 0.0, "other": {"anies": [{"value": "1.27064451379E-5", "module": "A1", "scenario": "Standard scenario"}, {"value": "1.13093548007E-5", "module": "A2", "scenario": "Standard scenario"}, {"value": "5.32141569066E-5", "module": "A3", "scenario": "Standard scenario"}, {"value": "2.66037052911E-5", "module": "A4", "scenario": "Standard scenario"}, {"value": "1.27482881757E-5", "module": "A5", "scenario": "Standard scenario"}, {"value": "0.0", "module": "C1", "scenario": "Standard scenario"}, {"value": "3.5784788426E-6", "module": "C2", "scenario": "Standard scenario"}, {"value": "0.0", "module": "C3", "scenario": "Standard scenario"}, {"value": "1.52636E-6", "module": "C4", "scenario": "Standard scenario"}, {"value": "-9.8629436031E-6", "module": "D", "scenario": "Standard scenario"}, {"name": "referenceToUnitGroupDataSet", "value": {"shortDescription": [{"value": "kg"}], "type": "unit group data set", "refObjectId": "ad38d542-3fe9-439d-9b95-2f5f7752acaf", "uri": "../unitgroups/ad38d542-3fe9-439d-9b95-2f5f7752acaf"}}]}, "resolvedFlowVersion": "38.00.000", "flowProperties": [], "typeOfFlow": "Other flow", "classification": {"classHierarchy": "Quantities / Environmental quantities / EPD EN 15804 / LCI indicators", "name": "GaBiCategories"}}, {"dataSetInternalID": 6, "referenceToFlowDataSet": {"shortDescription": [{"value": "Stoffe für die Energierückgewinnung (MER)", "lang": "de"}, {"value": "Materials for energy recovery (MER)", "lang": "en"}, {"value": "Materiales para valorización energética (recuperación de energía) (MER)", "lang": "es"}, {"value": "Material till energiåtervinning (MER)", "lang": "sv"}], "type": "flow data set", "refObjectId": "59a9181c-3aaf-46ee-8b13-2b3723b6e447", "version": "30.00.002"}, "exchange direction": "OUTPUT", "meanAmount": 0.0, "other": {"anies": [{"value": "0.0", "module": "A1", "scenario": "Standard scenario"}, {"value": "0.0", "module": "A2", "scenario": "Standard scenario"}, {"value": "0.0", "module": "A3", "scenario": "Standard scenario"}, {"value": "0.0", "module": "A4", "scenario": "Standard scenario"}, {"value": "0.0", "module": "A5", "scenario": "Standard scenario"}, {"value": "0.0", "module": "C1", "scenario": "Standard scenario"}, {"value": "0.0", "module": "C2", "scenario": "Standard scenario"}, {"value": "0.0", "module": "C3", "scenario": "Standard scenario"}, {"value": "0.0", "module": "C4", "scenario": "Standard scenario"}, {"value": "0.0", "module": "D", "scenario": "Standard scenario"}, {"name": "referenceToUnitGroupDataSet", "value": {"shortDescription": [{"value": "kg"}], "type": "unit group data set", "refObjectId": "ad38d542-3fe9-439d-9b95-2f5f7752acaf", "uri": "../unitgroups/ad38d542-3fe9-439d-9b95-2f5f7752acaf"}}]}, "resolvedFlowVersion": "38.00.000", "flowProperties": [], "typeOfFlow": "Other flow", "classification": {"classHierarchy": "Quantities / Environmental quantities / EPD EN 15804 / LCI indicators", "name": "GaBiCategories"}}, {"dataSetInternalID": 7, "referenceToFlowDataSet": {"shortDescription": [{"value": "Stoffe zum Recycling (MFR)", "lang": "de"}, {"value": "Materials for recycling (MFR)", "lang": "en"}, {"value": "Materiales para el reciclaje (MFR)", "lang": "es"}, {"value": "Material till återvinning (MFR)", "lang": "sv"}], "type": "flow data set", "refObjectId": "d7fe48a5-4103-49c8-9aae-b0b5dfdbd6ae", "version": "30.00.002"}, "exchange direction": "OUTPUT", "meanAmount": 0.0, "other": {"anies": [{"value": "0.0", "module": "A1", "scenario": "Standard scenario"}, {"value": "0.0", "module": "A2", "scenario": "Standard scenario"}, {"value": "0.0", "module": "A3", "scenario": "Standard scenario"}, {"value": "0.0", "module": "A4", "scenario": "Standard scenario"}, {"value": "0.2010795", "module": "A5", "scenario": "Standard scenario"}, {"value": "0.0", "module": "C1", "scenario": "Standard scenario"}, {"value": "0.0", "module": "C2", "scenario": "Standard scenario"}, {"value": "0.0", "module": "C3", "scenario": "Standard scenario"}, {"value": "0.0", "module": "C4", "scenario": "Standard scenario"}, {"value": "0.0", "module": "D", "scenario": "Standard scenario"}, {"name": "referenceToUnitGroupDataSet", "value": {"shortDescription": [{"value": "kg"}], "type": "unit group data set", "refObjectId": "ad38d542-3fe9-439d-9b95-2f5f7752acaf", "uri": "../unitgroups/ad38d542-3fe9-439d-9b95-2f5f7752acaf"}}]}, "resolvedFlowVersion": "38.00.000", "flowProperties": [], "typeOfFlow": "Other flow", "classification": {"classHierarchy": "Quantities / Environmental quantities / EPD EN 15804 / LCI indicators", "name": "GaBiCategories"}}, {"dataSetInternalID": 8, "referenceToFlowDataSet": {"shortDescription": [{"value": "Einsatz von Süßwasserressourcen (FW)", "lang": "de"}, {"value": "Use of net fresh water (FW)", "lang": "en"}, {"value": "Uso neto de recursos de agua dulce (FW)", "lang": "es"}, {"value": "Användning av sötvatten (FW)", "lang": "sv"}], "type": "flow data set", "refObjectId": "3cf952c8-f3a4-461d-8c96-96456ca62246", "version": "30.00.003"}, "exchange direction": "INPUT", "meanAmount": 0.0, "other": {"anies": [{"value": "0.0268044143658395", "module": "A1", "scenario": "Standard scenario"}, {"value": "5.43632288321E-4", "module": "A2", "scenario": "Standard scenario"}, {"value": "0.0072332764755612", "module": "A3", "scenario": "Standard scenario"}, {"value": "0.0012788203606686", "module": "A4", "scenario": "Standard scenario"}, {"value": "0.0026104067646437", "module": "A5", "scenario": "Standard scenario"}, {"value": "0.0", "module": "C1", "scenario": "Standard scenario"}, {"value": "1.720148210207E-4", "module": "C2", "scenario": "Standard scenario"}, {"value": "0.0", "module": "C3", "scenario": "Standard scenario"}, {"value": "0.001089266", "module": "C4", "scenario": "Standard scenario"}, {"value": "-4.361806433394E-4", "module": "D", "scenario": "Standard scenario"}, {"name": "referenceToUnitGroupDataSet", "value": {"shortDescription": [{"value": "m3"}], "type": "unit group data set", "refObjectId": "cd950537-0a98-4044-9ba7-9f9a68d0a504", "uri": "../unitgroups/cd950537-0a98-4044-9ba7-9f9a68d0a504"}}]}, "resolvedFlowVersion": "38.00.000", "flowProperties": [], "typeOfFlow": "Other flow", "classification": {"classHierarchy": "Quantities / Environmental quantities / EPD EN 15804 / LCI indicators", "name": "GaBiCategories"}}, {"dataSetInternalID": 9, "referenceToFlowDataSet": {"shortDescription": [{"value": "Entsorgter nicht gefährlicher Abfall (NHWD)", "lang": "de"}, {"value": "Non hazardous waste dispose (NHWD)", "lang": "en"}, {"value": "Residuos no peligrosos eliminados (NHWD)", "lang": "es"}, {"value": "Icke-farligt avfall (NHWD)", "lang": "sv"}], "type": "flow data set", "refObjectId": "b29ef66b-e286-4afa-949f-62f1a7b4d7fa", "version": "30.00.002"}, "exchange direction": "OUTPUT", "meanAmount": 0.0, "other": {"anies": [{"value": "0.177393115785156", "module": "A1", "scenario": "Standard scenario"}, {"value": "0.283095750000452", "module": "A2", "scenario": "Standard scenario"}, {"value": "0.365974781639504", "module": "A3", "scenario": "Standard scenario"}, {"value": "0.665943905277366", "module": "A4", "scenario": "Standard scenario"}, {"value": "0.460143089408178", "module": "A5", "scenario": "Standard scenario"}, {"value": "0.0", "module": "C1", "scenario": "Standard scenario"}, {"value": "0.0895764762583341", "module": "C2", "scenario": "Standard scenario"}, {"value": "0.0", "module": "C3", "scenario": "Standard scenario"}, {"value": "6.93588390999999", "module": "C4", "scenario": "Standard scenario"}, {"value": "-0.0331397115496007", "module": "D", "scenario": "Standard scenario"}, {"name": "referenceToUnitGroupDataSet", "value": {"shortDescription": [{"value": "kg"}], "type": "unit group data set", "refObjectId": "ad38d542-3fe9-439d-9b95-2f5f7752acaf", "uri": "../unitgroups/ad38d542-3fe9-439d-9b95-2f5f7752acaf"}}]}, "resolvedFlowVersion": "38.00.000", "flowProperties": [], "typeOfFlow": "Other flow", "classification": {"classHierarchy": "Quantities / Environmental quantities / EPD EN 15804 / LCI indicators", "name": "GaBiCategories"}}, {"dataSetInternalID": 10, "referenceToFlowDataSet": {"shortDescription": [{"value": "Nicht-erneuerbare Primärenergie als Energieträger (PENRE)", "lang": "de"}, {"value": "Use of non renewable primary energy (PENRE)", "lang": "en"}, {"value": "Uso de energía primaria no renovable, excluyendo los recursos de energía primaria no renovable utilizada como materia prima (PENRE)", "lang": "es"}, {"value": "Icke förnybar primärenergi - använd som energibärare (PENRE)", "lang": "sv"}], "type": "flow data set", "refObjectId": "ac857178-2b45-46ec-892a-a9a4332f0372", "version": "30.00.002"}, "exchange direction": "INPUT", "meanAmount": 0.0, "other": {"anies": [{"value": "54.3868509822356", "module": "A1", "scenario": "Standard scenario"}, {"value": "4.73837528404371", "module": "A2", "scenario": "Standard scenario"}, {"value": "40.4088914498435", "module": "A3", "scenario": "Standard scenario"}, {"value": "11.1463776525107", "module": "A4", "scenario": "Standard scenario"}, {"value": "5.68472190206415", "module": "A5", "scenario": "Standard scenario"}, {"value": "0.0", "module": "C1", "scenario": "Standard scenario"}, {"value": "1.49930530971779", "module": "C2", "scenario": "Standard scenario"}, {"value": "0.0", "module": "C3", "scenario": "Standard scenario"}, {"value": "1.084936688", "module": "C4", "scenario": "Standard scenario"}, {"value": "-1.5845933086861", "module": "D", "scenario": "Standard scenario"}, {"name": "referenceToUnitGroupDataSet", "value": {"shortDescription": [{"value": "MJ"}], "type": "unit group data set", "refObjectId": "93a60a57-a3c8-11da-a746-0800200c9a66", "uri": "../unitgroups/93a60a57-a3c8-11da-a746-0800200c9a66"}}]}, "resolvedFlowVersion": "38.00.000", "flowProperties": [], "typeOfFlow": "Other flow", "classification": {"classHierarchy": "Quantities", "name": "GaBiCategories"}}, {"dataSetInternalID": 11, "referenceToFlowDataSet": {"shortDescription": [{"value": "Nicht-erneuerbare Primärenergie zur stofflichen Nutzung (PENRM)", "lang": "de"}, {"value": "Use of non renewable primary energy resources used as raw materials (PENRM)", "lang": "en"}, {"value": "Uso de la energía primaria no renovable utilizada como materia prima (PENRM)", "lang": "es"}, {"value": "Icke förnybar primärenergi - använd som råmaterial (PENRM)", "lang": "sv"}], "type": "flow data set", "refObjectId": "1421caa0-679d-4bf4-b282-0eb850ccae27", "version": "30.00.001"}, "exchange direction": "INPUT", "meanAmount": 0.0, "other": {"anies": [{"value": "14.4398", "module": "A1", "scenario": "Standard scenario"}, {"value": "0.0", "module": "A2", "scenario": "Standard scenario"}, {"value": "0.759066", "module": "A3", "scenario": "Standard scenario"}, {"value": "0.0", "module": "A4", "scenario": "Standard scenario"}, {"value": "0.45596598", "module": "A5", "scenario": "Standard scenario"}, {"value": "0.0", "module": "C1", "scenario": "Standard scenario"}, {"value": "0.0", "module": "C2", "scenario": "Standard scenario"}, {"value": "0.0", "module": "C3", "scenario": "Standard scenario"}, {"value": "0.0", "module": "C4", "scenario": "Standard scenario"}, {"value": "-0.0117234188", "module": "D", "scenario": "Standard scenario"}, {"name": "referenceToUnitGroupDataSet", "value": {"shortDescription": [{"value": "MJ"}], "type": "unit group data set", "refObjectId": "93a60a57-a3c8-11da-a746-0800200c9a66", "uri": "../unitgroups/93a60a57-a3c8-11da-a746-0800200c9a66"}}]}, "resolvedFlowVersion": "38.00.000", "flowProperties": [], "typeOfFlow": "Other flow", "classification": {"classHierarchy": "Quantities", "name": "GaBiCategories"}}, {"dataSetInternalID": 12, "referenceToFlowDataSet": {"shortDescription": [{"value": "Nicht erneuerbare Sekundärbrennstoffe (NRSF)", "lang": "de"}, {"value": "Use of non renewable secondary fuels (NRSF)", "lang": "en"}, {"value": "Uso de combustibles secundarios no renovables (NRSF)", "lang": "es"}, {"value": "Användning av ickeförnybara sekundära bränslen (NRSF)", "lang": "sv"}], "type": "flow data set", "refObjectId": "89def144-d39a-4287-b86f-efde453ddcb2", "version": "30.00.001"}, "exchange direction": "INPUT", "meanAmount": 0.0, "other": {"anies": [{"value": "0.0", "module": "A1", "scenario": "Standard scenario"}, {"value": "0.0", "module": "A2", "scenario": "Standard scenario"}, {"value": "0.0", "module": "A3", "scenario": "Standard scenario"}, {"value": "0.0", "module": "A4", "scenario": "Standard scenario"}, {"value": "0.0", "module": "A5", "scenario": "Standard scenario"}, {"value": "0.0", "module": "C1", "scenario": "Standard scenario"}, {"value": "0.0", "module": "C2", "scenario": "Standard scenario"}, {"value": "0.0", "module": "C3", "scenario": "Standard scenario"}, {"value": "0.0", "module": "C4", "scenario": "Standard scenario"}, {"value": "0.0", "module": "D", "scenario": "Standard scenario"}, {"name": "referenceToUnitGroupDataSet", "value": {"shortDescription": [{"value": "MJ"}], "type": "unit group data set", "refObjectId": "93a60a57-a3c8-11da-a746-0800200c9a66", "uri": "../unitgroups/93a60a57-a3c8-11da-a746-0800200c9a66"}}]}, "resolvedFlowVersion": "38.00.000", "flowProperties": [], "typeOfFlow": "Other flow", "classification": {"classHierarchy": "Quantities / Environmental quantities / EPD EN 15804 / LCI indicators", "name": "GaBiCategories"}}, {"dataSetInternalID": 13, "referenceToFlowDataSet": {"shortDescription": [{"value": "Entsorgter radioaktiver Abfall (RWD)", "lang": "de"}, {"value": "Radioactive waste disposed (RWD)", "lang": "en"}, {"value": "Residuos radiactivos eliminados (RWD)", "lang": "es"}, {"value": "Radioaktivt avfall (RWD) ", "lang": "sv"}], "type": "flow data set", "refObjectId": "3449546e-52ad-4b39-b809-9fb77cea8ff6", "version": "30.00.001"}, "exchange direction": "OUTPUT", "meanAmount": 0.0, "other": {"anies": [{"value": "4.488836150255E-4", "module": "A1", "scenario": "Standard scenario"}, {"value": "2.93060875864E-5", "module": "A2", "scenario": "Standard scenario"}, {"value": "6.2036965481E-5", "module": "A3", "scenario": "Standard scenario"}, {"value": "6.89385496451E-5", "module": "A4", "scenario": "Standard scenario"}, {"value": "2.61222341204E-5", "module": "A5", "scenario": "Standard scenario"}, {"value": "0.0", "module": "C1", "scenario": "Standard scenario"}, {"value": "9.2729617414E-6", "module": "C2", "scenario": "Standard scenario"}, {"value": "0.0", "module": "C3", "scenario": "Standard scenario"}, {"value": "6.709046E-6", "module": "C4", "scenario": "Standard scenario"}, {"value": "-4.7578668504E-6", "module": "D", "scenario": "Standard scenario"}, {"name": "referenceToUnitGroupDataSet", "value": {"shortDescription": [{"value": "kg"}], "type": "unit group data set", "refObjectId": "ad38d542-3fe9-439d-9b95-2f5f7752acaf", "uri": "../unitgroups/ad38d542-3fe9-439d-9b95-2f5f7752acaf"}}]}, "resolvedFlowVersion": "38.00.000", "flowProperties": [], "typeOfFlow": "Other flow", "classification": {"classHierarchy": "Quantities / Environmental quantities / EPD EN 15804 / LCI indicators", "name": "GaBiCategories"}}, {"dataSetInternalID": 14, "referenceToFlowDataSet": {"shortDescription": [{"value": "Erneuerbare Primärenergie als Energieträger (PERE)", "lang": "de"}, {"value": "Use of renewable primary energy (PERE)", "lang": "en"}, {"value": "Uso de energía primaria renovable excluyendo los recursos de energía primaria renovable utilizada como materia prima (PERE)", "lang": "es"}, {"value": "Förnybar energi - använd som energibärare (PERE)", "lang": "sv"}], "type": "flow data set", "refObjectId": "20f32be5-0398-4288-9b6d-accddd195317", "version": "30.00.001"}, "exchange direction": "INPUT", "meanAmount": 0.0, "other": {"anies": [{"value": "10.9364800644922", "module": "A1", "scenario": "Standard scenario"}, {"value": "0.0558724021244583", "module": "A2", "scenario": "Standard scenario"}, {"value": "25.7365962139925", "module": "A3", "scenario": "Standard scenario"}, {"value": "0.131432159147319", "module": "A4", "scenario": "Standard scenario"}, {"value": "1.26626999563198", "module": "A5", "scenario": "Standard scenario"}, {"value": "0.0", "module": "C1", "scenario": "Standard scenario"}, {"value": "0.0176790110850821", "module": "C2", "scenario": "Standard scenario"}, {"value": "0.0", "module": "C3", "scenario": "Standard scenario"}, {"value": "0.00825622", "module": "C4", "scenario": "Standard scenario"}, {"value": "-15.8385242814874", "module": "D", "scenario": "Standard scenario"}, {"name": "referenceToUnitGroupDataSet", "value": {"shortDescription": [{"value": "MJ"}], "type": "unit group data set", "refObjectId": "93a60a57-a3c8-11da-a746-0800200c9a66", "uri": "../unitgroups/93a60a57-a3c8-11da-a746-0800200c9a66"}}]}, "resolvedFlowVersion": "38.00.000", "flowProperties": [], "typeOfFlow": "Other flow", "classification": {"classHierarchy": "Quantities", "name": "GaBiCategories"}}, {"dataSetInternalID": 15, "referenceToFlowDataSet": {"shortDescription": [{"value": "Erneuerbare Primärenergie zur stofflichen Nutzung (PERM)", "lang": "de"}, {"value": "Use of renewable primary energy resources used as raw materials (PERM)", "lang": "en"}, {"value": "Uso de energía primaria renovable utilizada como materia prima (PERM)", "lang": "es"}, {"value": "Förnybar energi - använd som råmaterial (PERM)", "lang": "sv"}], "type": "flow data set", "refObjectId": "fb3ec0de-548d-4508-aea5-00b73bf6f702", "version": "30.00.001"}, "exchange direction": "INPUT", "meanAmount": 0.0, "other": {"anies": [{"value": "0.0", "module": "A1", "scenario": "Standard scenario"}, {"value": "0.0", "module": "A2", "scenario": "Standard scenario"}, {"value": "16.3739583999999", "module": "A3", "scenario": "Standard scenario"}, {"value": "0.0", "module": "A4", "scenario": "Standard scenario"}, {"value": "0.491218752", "module": "A5", "scenario": "Standard scenario"}, {"value": "0.0", "module": "C1", "scenario": "Standard scenario"}, {"value": "0.0", "module": "C2", "scenario": "Standard scenario"}, {"value": "0.0", "module": "C3", "scenario": "Standard scenario"}, {"value": "0.0", "module": "C4", "scenario": "Standard scenario"}, {"value": "0.0", "module": "D", "scenario": "Standard scenario"}, {"name": "referenceToUnitGroupDataSet", "value": {"shortDescription": [{"value": "MJ"}], "type": "unit group data set", "refObjectId": "93a60a57-a3c8-11da-a746-0800200c9a66", "uri": "../unitgroups/93a60a57-a3c8-11da-a746-0800200c9a66"}}]}, "resolvedFlowVersion": "38.00.000", "flowProperties": [], "typeOfFlow": "Other flow", "classification": {"classHierarchy": "Quantities", "name": "GaBiCategories"}}, {"dataSetInternalID": 16, "referenceToFlowDataSet": {"shortDescription": [{"value": "Erneuerbare Sekundärbrennstoffe (RSF)", "lang": "de"}, {"value": "Use of renewable secondary fuels (RSF)", "lang": "en"}, {"value": "Uso de combustibles secundarios renovables (RSF)", "lang": "es"}, {"value": "Användning av förnybara sekundära bränslen (RSF)", "lang": "sv"}], "type": "flow data set", "refObjectId": "64333088-a55f-4aa2-9a31-c10b07816787", "version": "30.00.001"}, "exchange direction": "INPUT", "meanAmount": 0.0, "other": {"anies": [{"value": "0.0", "module": "A1", "scenario": "Standard scenario"}, {"value": "0.0", "module": "A2", "scenario": "Standard scenario"}, {"value": "0.0", "module": "A3", "scenario": "Standard scenario"}, {"value": "0.0", "module": "A4", "scenario": "Standard scenario"}, {"value": "0.0", "module": "A5", "scenario": "Standard scenario"}, {"value": "0.0", "module": "C1", "scenario": "Standard scenario"}, {"value": "0.0", "module": "C2", "scenario": "Standard scenario"}, {"value": "0.0", "module": "C3", "scenario": "Standard scenario"}, {"value": "0.0", "module": "C4", "scenario": "Standard scenario"}, {"value": "0.0", "module": "D", "scenario": "Standard scenario"}, {"name": "referenceToUnitGroupDataSet", "value": {"shortDescription": [{"value": "MJ"}], "type": "unit group data set", "refObjectId": "93a60a57-a3c8-11da-a746-0800200c9a66", "uri": "../unitgroups/93a60a57-a3c8-11da-a746-0800200c9a66"}}]}, "resolvedFlowVersion": "38.00.000", "flowProperties": [], "typeOfFlow": "Other flow", "classification": {"classHierarchy": "Quantities / Environmental quantities / EPD EN 15804 / LCI indicators", "name": "GaBiCategories"}}, {"dataSetInternalID": 17, "referenceToFlowDataSet": {"shortDescription": [{"value": "Einsatz von Sekundärstoffen (SM)", "lang": "de"}, {"value": "Use of secondary material (SM)", "lang": "en"}, {"value": "Uso de materiales secundarios (SM)", "lang": "es"}, {"value": "Användning av sekundära material (SM)", "lang": "sv"}], "type": "flow data set", "refObjectId": "c6a1f35f-2d09-4f54-8dfb-97e502e1ce92", "version": "30.00.001"}, "exchange direction": "INPUT", "meanAmount": 0.0, "other": {"anies": [{"value": "8.11465999999999", "module": "A1", "scenario": "Standard scenario"}, {"value": "0.0", "module": "A2", "scenario": "Standard scenario"}, {"value": "0.2434398", "module": "A3", "scenario": "Standard scenario"}, {"value": "0.0", "module": "A4", "scenario": "Standard scenario"}, {"value": "0.290165102863976", "module": "A5", "scenario": "Standard scenario"}, {"value": "0.0", "module": "C1", "scenario": "Standard scenario"}, {"value": "0.0", "module": "C2", "scenario": "Standard scenario"}, {"value": "0.0", "module": "C3", "scenario": "Standard scenario"}, {"value": "0.0", "module": "C4", "scenario": "Standard scenario"}, {"value": "0.0", "module": "D", "scenario": "Standard scenario"}, {"name": "referenceToUnitGroupDataSet", "value": {"shortDescription": [{"value": "kg"}], "type": "unit group data set", "refObjectId": "ad38d542-3fe9-439d-9b95-2f5f7752acaf", "uri": "../unitgroups/ad38d542-3fe9-439d-9b95-2f5f7752acaf"}}]}, "resolvedFlowVersion": "38.00.000", "flowProperties": [], "typeOfFlow": "Other flow", "classification": {"classHierarchy": "Quantities / Environmental quantities / EPD EN 15804 / LCI indicators", "name": "GaBiCategories"}}, {"dataSetInternalID": 18, "referenceToFlowDataSet": {"shortDescription": [{"value": "Total nicht erneuerbare Primärenergie (PENRT)", "lang": "de"}, {"value": "Total use of non renewable primary energy resource (PENRT)", "lang": "en"}, {"value": "Uso total de la energía primaria no renovable (energía primaria y recursos de energía primaria renovable utilizada como materia prima) (PENRT)", "lang": "es"}, {"value": "Icke förnybar primärenergi – total (PENRT)", "lang": "sv"}], "type": "flow data set", "refObjectId": "06159210-646b-4c8d-8583-da9b3b95a6c1", "version": "30.00.001"}, "exchange direction": "INPUT", "meanAmount": 0.0, "other": {"anies": [{"value": "68.8266509822356", "module": "A1", "scenario": "Standard scenario"}, {"value": "4.73837528404371", "module": "A2", "scenario": "Standard scenario"}, {"value": "41.1679574498435", "module": "A3", "scenario": "Standard scenario"}, {"value": "11.1463776525107", "module": "A4", "scenario": "Standard scenario"}, {"value": "6.14068788206416", "module": "A5", "scenario": "Standard scenario"}, {"value": "0.0", "module": "C1", "scenario": "Standard scenario"}, {"value": "1.49930530971779", "module": "C2", "scenario": "Standard scenario"}, {"value": "0.0", "module": "C3", "scenario": "Standard scenario"}, {"value": "1.084936688", "module": "C4", "scenario": "Standard scenario"}, {"value": "-1.5963167274861", "module": "D", "scenario": "Standard scenario"}, {"name": "referenceToUnitGroupDataSet", "value": {"shortDescription": [{"value": "MJ"}], "type": "unit group data set", "refObjectId": "93a60a57-a3c8-11da-a746-0800200c9a66", "uri": "../unitgroups/93a60a57-a3c8-11da-a746-0800200c9a66"}}]}, "resolvedFlowVersion": "38.00.000", "flowProperties": [], "typeOfFlow": "Other flow", "classification": {"classHierarchy": "Quantities / Environmental quantities / EPD EN 15804 / LCI indicators", "name": "GaBiCategories"}}, {"dataSetInternalID": 19, "referenceToFlowDataSet": {"shortDescription": [{"value": "Total erneuerbare Primärenergie (PERT)", "lang": "de"}, {"value": "Total use of renewable primary energy resources (PERT)", "lang": "en"}, {"value": "Uso total de la energía primaria renovable (energía primaria y recursos de energía primaria renovable utilizada como materia prima) (PERT)", "lang": "es"}, {"value": "Förnybar energi – total (PERT)", "lang": "sv"}], "type": "flow data set", "refObjectId": "53f97275-fa8a-4cdd-9024-65936002acd0", "version": "30.00.001"}, "exchange direction": "INPUT", "meanAmount": 0.0, "other": {"anies": [{"value": "10.9364800644922", "module": "A1", "scenario": "Standard scenario"}, {"value": "0.0558724021244583", "module": "A2", "scenario": "Standard scenario"}, {"value": "42.1105546139925", "module": "A3", "scenario": "Standard scenario"}, {"value": "0.131432159147319", "module": "A4", "scenario": "Standard scenario"}, {"value": "1.75748874763198", "module": "A5", "scenario": "Standard scenario"}, {"value": "0.0", "module": "C1", "scenario": "Standard scenario"}, {"value": "0.0176790110850821", "module": "C2", "scenario": "Standard scenario"}, {"value": "0.0", "module": "C3", "scenario": "Standard scenario"}, {"value": "0.00825622", "module": "C4", "scenario": "Standard scenario"}, {"value": "-15.8385242814874", "module": "D", "scenario": "Standard scenario"}, {"name": "referenceToUnitGroupDataSet", "value": {"shortDescription": [{"value": "MJ"}], "type": "unit group data set", "refObjectId": "93a60a57-a3c8-11da-a746-0800200c9a66", "uri": "../unitgroups/93a60a57-a3c8-11da-a746-0800200c9a66"}}]}, "resolvedFlowVersion": "38.00.000", "flowProperties": [], "typeOfFlow": "Other flow", "classification": {"classHierarchy": "Quantities / Environmental quantities / EPD EN 15804 / LCI indicators", "name": "GaBiCategories"}}]}, "LCIAResults": {"LCIAResult": [{"referenceToLCIAMethodDataSet": {"shortDescription": [{"value": "Potenzial für die Verknappung abiotischer Ressourcen – nicht fossile Ressourcen (ADPE)", "lang": "de"}, {"value": "Abiotic depletion potential - non-fossil resources (ADPE)", "lang": "en"}, {"value": "Abiotisk utarmningspotential icke fossila resurser (ADP-mm)", "lang": "sv"}], "type": "LCIA method data set", "refObjectId": "b2ad6494-c78d-11e6-9d9d-cec0c932ce01", "version": "01.00.012"}, "meanAmount": 0.0, "other": {"anies": [{"value": "3.51849749027E-5", "module": "A1", "scenario": "Standard scenario"}, {"value": "7.4974486505E-6", "module": "A2", "scenario": "Standard scenario"}, {"value": "1.2690998391E-5", "module": "A3", "scenario": "Standard scenario"}, {"value": "1.7636719145E-5", "module": "A4", "scenario": "Standard scenario"}, {"value": "5.5749739015E-6", "module": "A5", "scenario": "Standard scenario"}, {"value": "0.0", "module": "C1", "scenario": "Standard scenario"}, {"value": "2.3723246677E-6", "module": "C2", "scenario": "Standard scenario"}, {"value": "0.0", "module": "C3", "scenario": "Standard scenario"}, {"value": "3.344116E-7", "module": "C4", "scenario": "Standard scenario"}, {"value": "-9.581911579E-7", "module": "D", "scenario": "Standard scenario"}, {"name": "referenceToUnitGroupDataSet", "value": {"shortDescription": [{"value": "kg Sb-Äqv."}], "type": "unit group data set", "refObjectId": "54ccd2d9-a32a-4fc2-923d-f2c8c93e89d4", "uri": "../unitgroups/54ccd2d9-a32a-4fc2-923d-f2c8c93e89d4"}}]}}, {"referenceToLCIAMethodDataSet": {"shortDescription": [{"value": "Potenzial für die Verknappung abiotischer Ressourcen – fossile Brennstoffe (ADPF)", "lang": "de"}, {"value": "Abiotic depletion potential - fossil resources (ADPF)", "lang": "en"}, {"value": "Abiotisk utarmningspotential av fossila resurser (ADP-F)", "lang": "sv"}], "type": "LCIA method data set", "refObjectId": "b2ad6110-c78d-11e6-9d9d-cec0c932ce01", "version": "01.00.012"}, "meanAmount": 0.0, "other": {"anies": [{"value": "66.287562733814", "module": "A1", "scenario": "Standard scenario"}, {"value": "4.46290545031415", "module": "A2", "scenario": "Standard scenario"}, {"value": "37.6128457389249", "module": "A3", "scenario": "Standard scenario"}, {"value": "10.498372668827", "module": "A4", "scenario": "Standard scenario"}, {"value": "5.79330480024766", "module": "A5", "scenario": "Standard scenario"}, {"value": "0.0", "module": "C1", "scenario": "Standard scenario"}, {"value": "1.41214180754256", "module": "C2", "scenario": "Standard scenario"}, {"value": "0.0", "module": "C3", "scenario": "Standard scenario"}, {"value": "1.02139154599999", "module": "C4", "scenario": "Standard scenario"}, {"value": "-1.49733534810948", "module": "D", "scenario": "Standard scenario"}, {"name": "referenceToUnitGroupDataSet", "value": {"shortDescription": [{"value": "MJ"}], "type": "unit group data set", "refObjectId": "93a60a57-a3c8-11da-a746-0800200c9a66", "uri": "../unitgroups/93a60a57-a3c8-11da-a746-0800200c9a66"}}]}}, {"referenceToLCIAMethodDataSet": {"shortDescription": [{"value": "Versauerungspotenzial, kumulierte Überschreitung (AP)", "lang": "de"}, {"value": "Acidification potential, Accumulated Exceedance (AP)", "lang": "en"}, {"value": "Försurningspotential på land och vatten (AP)", "lang": "sv"}], "type": "LCIA method data set", "refObjectId": "b5c611c6-def3-11e6-bf01-fe55135034f3", "version": "01.03.011", "uri": "http://lca.jrc.ec.europa.eu/lcainfohub/datasets/elcd/lciamethods/f6cbd466-253f-4145-a4bb-8dae7d266e89.xml"}, "meanAmount": 0.0, "other": {"anies": [{"value": "0.0111858842191905", "module": "A1", "scenario": "Standard scenario"}, {"value": "0.0017161976088601", "module": "A2", "scenario": "Standard scenario"}, {"value": "0.0051510339549985", "module": "A3", "scenario": "Standard scenario"}, {"value": "0.0040371193769958", "module": "A4", "scenario": "Standard scenario"}, {"value": "0.0019246089333847", "module": "A5", "scenario": "Standard scenario"}, {"value": "0.0", "module": "C1", "scenario": "Standard scenario"}, {"value": "5.430351192641E-4", "module": "C2", "scenario": "Standard scenario"}, {"value": "0.0", "module": "C3", "scenario": "Standard scenario"}, {"value": "3.469E-4", "module": "C4", "scenario": "Standard scenario"}, {"value": "-0.002100943457389", "module": "D", "scenario": "Standard scenario"}, {"name": "referenceToUnitGroupDataSet", "value": {"shortDescription": [{"value": "mol H+ eqv."}], "type": "unit group data set", "refObjectId": "42e089ac-92bf-4bf2-8ca1-5fc40d18f2ed", "uri": "../unitgroups/42e089ac-92bf-4bf2-8ca1-5fc40d18f2ed"}}]}}, {"referenceToLCIAMethodDataSet": {"shortDescription": [{"value": "Eutrophierungspotenzial - Süßwasser (EP-freshwater)", "lang": "de"}, {"value": "Eutrophication potential - freshwater (EP-freshwater)", "lang": "en"}, {"value": "Övergödningspotential sötvatten (EP-fw)", "lang": "sv"}], "type": "LCIA method data set", "refObjectId": "b53ec18f-7377-4ad3-86eb-cc3f4f276b2b", "version": "01.00.012", "uri": "http://lca.jrc.ec.europa.eu/lcainfohub/datasets/elcd/lciamethods/a4630d5b-df2f-48ae-b3f2-5e5257606d68.xml"}, "meanAmount": 0.0, "other": {"anies": [{"value": "7.64973657108E-5", "module": "A1", "scenario": "Standard scenario"}, {"value": "2.985028029E-6", "module": "A2", "scenario": "Standard scenario"}, {"value": "4.21564969836E-5", "module": "A3", "scenario": "Standard scenario"}, {"value": "7.0218688305E-6", "module": "A4", "scenario": "Standard scenario"}, {"value": "1.33432482263E-5", "module": "A5", "scenario": "Standard scenario"}, {"value": "0.0", "module": "C1", "scenario": "Standard scenario"}, {"value": "9.445153888E-7", "module": "C2", "scenario": "Standard scenario"}, {"value": "0.0", "module": "C3", "scenario": "Standard scenario"}, {"value": "4.09342E-7", "module": "C4", "scenario": "Standard scenario"}, {"value": "-8.4072115685E-6", "module": "D", "scenario": "Standard scenario"}, {"name": "referenceToUnitGroupDataSet", "value": {"shortDescription": [{"value": "kg P eqv."}], "type": "unit group data set", "refObjectId": "0429039d-a61d-4590-ba67-aa4a20a810a1", "uri": "../unitgroups/0429039d-a61d-4590-ba67-aa4a20a810a1"}}]}}, {"referenceToLCIAMethodDataSet": {"shortDescription": [{"value": "Eutrophierungspotenzial - Salzwasser (EP-marine)", "lang": "de"}, {"value": "Eutrophication potential - marine (EP-marine)", "lang": "en"}, {"value": "Övergödningspotential marin (EP-m)", "lang": "sv"}], "type": "LCIA method data set", "refObjectId": "b5c619fa-def3-11e6-bf01-fe55135034f3", "version": "02.00.012", "uri": "http://lca.jrc.ec.europa.eu/lcainfohub/datasets/elcd/lciamethods/5296e2be-060b-4e50-b033-d45f85f6ac92.xml"}, "meanAmount": 0.0, "other": {"anies": [{"value": "0.0030596291501107", "module": "A1", "scenario": "Standard scenario"}, {"value": "6.047468813459E-4", "module": "A2", "scenario": "Standard scenario"}, {"value": "0.0013126302980206", "module": "A3", "scenario": "Standard scenario"}, {"value": "0.0014225840545721", "module": "A4", "scenario": "Standard scenario"}, {"value": "5.693721331898E-4", "module": "A5", "scenario": "Standard scenario"}, {"value": "0.0", "module": "C1", "scenario": "Standard scenario"}, {"value": "1.91352553541E-4", "module": "C2", "scenario": "Standard scenario"}, {"value": "0.0", "module": "C3", "scenario": "Standard scenario"}, {"value": "1.193336E-4", "module": "C4", "scenario": "Standard scenario"}, {"value": "-5.898776070348E-4", "module": "D", "scenario": "Standard scenario"}, {"name": "referenceToUnitGroupDataSet", "value": {"shortDescription": [{"value": "kg N eqv."}], "type": "unit group data set", "refObjectId": "d05bb823-ecdf-4686-8c40-bf1d9257859f", "uri": "../unitgroups/d05bb823-ecdf-4686-8c40-bf1d9257859f"}}]}}, {"referenceToLCIAMethodDataSet": {"shortDescription": [{"value": "Eutrophierungspotenzial - Land (EP-terrestrial)", "lang": "de"}, {"value": "Eutrophication potential - terrestrial (EP-terrestrial)", "lang": "en"}, {"value": "Övergödningspotential total (EP-T)", "lang": "sv"}], "type": "LCIA method data set", "refObjectId": "b5c614d2-def3-11e6-bf01-fe55135034f3", "version": "01.02.011", "uri": "http://lca.jrc.ec.europa.eu/lcainfohub/datasets/elcd/lciamethods/40054970-5936-477c-9bec-29fa23b1cb77.xml"}, "meanAmount": 0.0, "other": {"anies": [{"value": "0.031889491463749", "module": "A1", "scenario": "Standard scenario"}, {"value": "0.0066674049945849", "module": "A2", "scenario": "Standard scenario"}, {"value": "0.0146640596240032", "module": "A3", "scenario": "Standard scenario"}, {"value": "0.01568415534374", "module": "A4", "scenario": "Standard scenario"}, {"value": "0.0062072910936219", "module": "A5", "scenario": "Standard scenario"}, {"value": "0.0", "module": "C1", "scenario": "Standard scenario"}, {"value": "0.0021096842506508", "module": "C2", "scenario": "Standard scenario"}, {"value": "0.0", "module": "C3", "scenario": "Standard scenario"}, {"value": "0.00131822", "module": "C4", "scenario": "Standard scenario"}, {"value": "-0.0094208948612891", "module": "D", "scenario": "Standard scenario"}, {"name": "referenceToUnitGroupDataSet", "value": {"shortDescription": [{"value": "mol N eqv."}], "type": "unit group data set", "refObjectId": "71b4d617-0ec9-4d3f-b65e-e438940c2401", "uri": "../unitgroups/71b4d617-0ec9-4d3f-b65e-e438940c2401"}}]}}, {"referenceToLCIAMethodDataSet": {"shortDescription": [{"value": "Globales Erwärmungspotenzial - total (GWP-total)", "lang": "de"}, {"value": "Global Warming Potential - total (GWP-total)", "lang": "en"}, {"value": "Global uppvärmningspotential – Totalt (GWP-T)", "lang": "sv"}], "type": "LCIA method data set", "refObjectId": "6a37f984-a4b3-458a-a20a-64418c145fa2", "version": "04.00.018"}, "meanAmount": 0.0, "other": {"anies": [{"value": "3.22037809211743", "module": "A1", "scenario": "Standard scenario"}, {"value": "0.296154617257973", "module": "A2", "scenario": "Standard scenario"}, {"value": "0.366609554894298", "module": "A3", "scenario": "Standard scenario"}, {"value": "0.6966630985537", "module": "A4", "scenario": "Standard scenario"}, {"value": "2.34813973863833", "module": "A5", "scenario": "Standard scenario"}, {"value": "0.0", "module": "C1", "scenario": "Standard scenario"}, {"value": "0.0937085316242385", "module": "C2", "scenario": "Standard scenario"}, {"value": "0.0", "module": "C3", "scenario": "Standard scenario"}, {"value": "0.036611826", "module": "C4", "scenario": "Standard scenario"}, {"value": "-0.143178712341303", "module": "D", "scenario": "Standard scenario"}, {"name": "referenceToUnitGroupDataSet", "value": {"shortDescription": [{"value": "kg CO2-Äqv."}], "type": "unit group data set", "refObjectId": "1ebf3012-d0db-4de2-aefd-ef30cedb0be1", "uri": "../unitgroups/1ebf3012-d0db-4de2-aefd-ef30cedb0be1"}}]}}, {"referenceToLCIAMethodDataSet": {"shortDescription": [{"value": "Globales Erwärmungspotenzial - fossil (GWP-fossil)", "lang": "de"}, {"value": "Global Warming Potential - fossil fuels (GWP-fossil)", "lang": "en"}, {"value": "Global uppvärmningspotential– fossil (GWP-f)", "lang": "sv"}], "type": "LCIA method data set", "refObjectId": "5f635281-343e-44fb-83df-1971b155e6b6", "version": "01.00.011"}, "meanAmount": 0.0, "other": {"anies": [{"value": "3.61185789382284", "module": "A1", "scenario": "Standard scenario"}, {"value": "0.295909579715029", "module": "A2", "scenario": "Standard scenario"}, {"value": "2.29926627174909", "module": "A3", "scenario": "Standard scenario"}, {"value": "0.696086681358147", "module": "A4", "scenario": "Standard scenario"}, {"value": "0.421944776483974", "module": "A5", "scenario": "Standard scenario"}, {"value": "0.0", "module": "C1", "scenario": "Standard scenario"}, {"value": "0.0936309974343118", "module": "C2", "scenario": "Standard scenario"}, {"value": "0.0", "module": "C3", "scenario": "Standard scenario"}, {"value": "0.036535508", "module": "C4", "scenario": "Standard scenario"}, {"value": "-0.137303961017088", "module": "D", "scenario": "Standard scenario"}, {"name": "referenceToUnitGroupDataSet", "value": {"shortDescription": [{"value": "kg CO2-Äqv."}], "type": "unit group data set", "refObjectId": "1ebf3012-d0db-4de2-aefd-ef30cedb0be1", "uri": "../unitgroups/1ebf3012-d0db-4de2-aefd-ef30cedb0be1"}}]}}, {"referenceToLCIAMethodDataSet": {"shortDescription": [{"value": "Globales Erwärmungspotenzial - biogen (GWP-biogenic)", "lang": "de"}, {"value": "Global Warming Potential - biogenic (GWP-biogenic)", "lang": "en"}, {"value": "Global uppvärmningspotential – biogen (GWP-b)", "lang": "sv"}], "type": "LCIA method data set", "refObjectId": "2356e1ab-0185-4db5-86e5-16de51c7485c", "version": "01.00.007"}, "meanAmount": 0.0, "other": {"anies": [{"value": "-0.394295217367158", "module": "A1", "scenario": "Standard scenario"}, {"value": "1.366062966114E-4", "module": "A2", "scenario": "Standard scenario"}, {"value": "-1.93534975131402", "module": "A3", "scenario": "Standard scenario"}, {"value": "3.213475675659E-4", "module": "A4", "scenario": "Standard scenario"}, {"value": "1.92590374691763", "module": "A5", "scenario": "Standard scenario"}, {"value": "0.0", "module": "C1", "scenario": "Standard scenario"}, {"value": "4.32246357818E-5", "module": "C2", "scenario": "Standard scenario"}, {"value": "0.0", "module": "C3", "scenario": "Standard scenario"}, {"value": "7.21552E-5", "module": "C4", "scenario": "Standard scenario"}, {"value": "-0.0052078787870375", "module": "D", "scenario": "Standard scenario"}, {"name": "referenceToUnitGroupDataSet", "value": {"shortDescription": [{"value": "kg CO2-Äqv."}], "type": "unit group data set", "refObjectId": "1ebf3012-d0db-4de2-aefd-ef30cedb0be1", "uri": "../unitgroups/1ebf3012-d0db-4de2-aefd-ef30cedb0be1"}}]}}, {"referenceToLCIAMethodDataSet": {"shortDescription": [{"value": "Globales Erwärmungspotenzial - luluc (GWP-luluc)", "lang": "de"}, {"value": "Global Warming Potential - land use and land use change (GWP-luluc)", "lang": "en"}, {"value": "Global uppvärmningspotential - markanvändning och förändringar i markanvändning (GWP-luluc)", "lang": "sv"}], "type": "LCIA method data set", "refObjectId": "4331bbdb-978a-490d-8707-eeb047f01a55", "version": "01.00.007"}, "meanAmount": 0.0, "other": {"anies": [{"value": "0.0028330722717512", "module": "A1", "scenario": "Standard scenario"}, {"value": "1.084312463332E-4", "module": "A2", "scenario": "Standard scenario"}, {"value": "0.0026916185723408", "module": "A3", "scenario": "Standard scenario"}, {"value": "2.550696279867E-4", "module": "A4", "scenario": "Standard scenario"}, {"value": "2.921867647283E-4", "module": "A5", "scenario": "Standard scenario"}, {"value": "0.0", "module": "C1", "scenario": "Standard scenario"}, {"value": "3.43095541449E-5", "module": "C2", "scenario": "Standard scenario"}, {"value": "0.0", "module": "C3", "scenario": "Standard scenario"}, {"value": "1.019886E-5", "module": "C4", "scenario": "Standard scenario"}, {"value": "-6.669924740316E-4", "module": "D", "scenario": "Standard scenario"}, {"name": "referenceToUnitGroupDataSet", "value": {"shortDescription": [{"value": "kg CO2-Äqv."}], "type": "unit group data set", "refObjectId": "1ebf3012-d0db-4de2-aefd-ef30cedb0be1", "uri": "../unitgroups/1ebf3012-d0db-4de2-aefd-ef30cedb0be1"}}]}}, {"referenceToLCIAMethodDataSet": {"shortDescription": [{"value": "Abbaupotenzial der stratosphärischen Ozonschicht (ODP)", "lang": "de"}, {"value": "Depletion potential of the stratospheric ozone layer (ODP)", "lang": "en"}, {"value": "Utarmningspotential för stratosfäriska ozonskiktet - ozonnedbrytning (ODP)", "lang": "sv"}], "type": "LCIA method data set", "refObjectId": "b5c629d6-def3-11e6-bf01-fe55135034f3", "version": "02.00.014", "uri": "http://lca.jrc.ec.europa.eu/lcainfohub/datasets/elcd/lciamethods/8b723200-3d8f-4eec-9e10-444edb029476.xml"}, "meanAmount": 0.0, "other": {"anies": [{"value": "6.46240619E-8", "module": "A1", "scenario": "Standard scenario"}, {"value": "6.5314351E-8", "module": "A2", "scenario": "Standard scenario"}, {"value": "2.891202293E-7", "module": "A3", "scenario": "Standard scenario"}, {"value": "1.536430481E-7", "module": "A4", "scenario": "Standard scenario"}, {"value": "3.5777511E-8", "module": "A5", "scenario": "Standard scenario"}, {"value": "0.0", "module": "C1", "scenario": "Standard scenario"}, {"value": "2.06666098E-8", "module": "C2", "scenario": "Standard scenario"}, {"value": "0.0", "module": "C3", "scenario": "Standard scenario"}, {"value": "1.505546E-8", "module": "C4", "scenario": "Standard scenario"}, {"value": "-2.10784961E-8", "module": "D", "scenario": "Standard scenario"}, {"name": "referenceToUnitGroupDataSet", "value": {"shortDescription": [{"value": "kg CFC 11-Äquiv."}], "type": "unit group data set", "refObjectId": "d9e957c9-7309-4474-bf3a-7777df6c4e5b", "uri": "../unitgroups/d9e957c9-7309-4474-bf3a-7777df6c4e5b"}}]}}, {"referenceToLCIAMethodDataSet": {"shortDescription": [{"value": "Bildungspotenzial für troposphärisches Ozon (POCP)", "lang": "de"}, {"value": "Photochemical Ozone Creation Potential (POCP)", "lang": "en"}, {"value": "Potential till fotokemisk oxidantbildning – marknära ozon (POCP)", "lang": "sv"}], "type": "LCIA method data set", "refObjectId": "b5c610fe-def3-11e6-bf01-fe55135034f3", "version": "02.00.017", "uri": "http://lca.jrc.ec.europa.eu/lcainfohub/datasets/elcd/lciamethods/ec7836be-83eb-41da-bcda-1a6a3fe2d149.xml"}, "meanAmount": 0.0, "other": {"anies": [{"value": "0.007851987041912", "module": "A1", "scenario": "Standard scenario"}, {"value": "0.001903592145828", "module": "A2", "scenario": "Standard scenario"}, {"value": "0.0051776691904666", "module": "A3", "scenario": "Standard scenario"}, {"value": "0.004477939310802", "module": "A4", "scenario": "Standard scenario"}, {"value": "0.001926087228759", "module": "A5", "scenario": "Standard scenario"}, {"value": "0.0", "module": "C1", "scenario": "Standard scenario"}, {"value": "6.023300478938E-4", "module": "C2", "scenario": "Standard scenario"}, {"value": "0.0", "module": "C3", "scenario": "Standard scenario"}, {"value": "3.822838E-4", "module": "C4", "scenario": "Standard scenario"}, {"value": "-0.0019196737799487", "module": "D", "scenario": "Standard scenario"}, {"name": "referenceToUnitGroupDataSet", "value": {"shortDescription": [{"value": "kg NMVOC eqv."}], "type": "unit group data set", "refObjectId": "d27c25f8-fbc1-44c6-b47b-4adbae4199c6", "uri": "../unitgroups/d27c25f8-fbc1-44c6-b47b-4adbae4199c6"}}]}}, {"referenceToLCIAMethodDataSet": {"shortDescription": [{"value": "Wasser-Entzugspotenzial (Benutzer) (WDP)", "lang": "de"}, {"value": "Water (user) deprivation potential (WDP)", "lang": "en"}, {"value": "Vattenfotavtryck (WDP)", "lang": "sv"}], "type": "LCIA method data set", "refObjectId": "b2ad66ce-c78d-11e6-9d9d-cec0c932ce01", "version": "03.00.016"}, "meanAmount": 0.0, "other": {"anies": [{"value": "0.852653772274978", "module": "A1", "scenario": "Standard scenario"}, {"value": "0.0159669135504648", "module": "A2", "scenario": "Standard scenario"}, {"value": "0.225788176875242", "module": "A3", "scenario": "Standard scenario"}, {"value": "0.0375599731363175", "module": "A4", "scenario": "Standard scenario"}, {"value": "0.0660502253439924", "module": "A5", "scenario": "Standard scenario"}, {"value": "0.0", "module": "C1", "scenario": "Standard scenario"}, {"value": "0.0050522123789206", "module": "C2", "scenario": "Standard scenario"}, {"value": "0.0", "module": "C3", "scenario": "Standard scenario"}, {"value": "0.045783862", "module": "C4", "scenario": "Standard scenario"}, {"value": "-0.0186958042512258", "module": "D", "scenario": "Standard scenario"}, {"name": "referenceToUnitGroupDataSet", "value": {"shortDescription": [{"value": "m3 world eqv."}], "type": "unit group data set", "refObjectId": "6ae2df01-888e-46c8-b17d-49fa3869b476", "uri": "../unitgroups/6ae2df01-888e-46c8-b17d-49fa3869b476"}}]}}, {"referenceToLCIAMethodDataSet": {"shortDescription": [{"value": "Potenzielles Auftreten von Krankheiten aufgrund von Feinstaubemissionen (PM)", "lang": "de"}, {"value": "Potential incidence of disease due to PM emissions (PM)", "lang": "en"}, {"value": "Potential till utsläpp av partiklar (PM)", "lang": "sv"}], "type": "LCIA method data set", "refObjectId": "b5c602c6-def3-11e6-bf01-fe55135034f3", "version": "02.00.013", "uri": "http://lca.jrc.ec.europa.eu/lcainfohub/datasets/elcd/lciamethods/72ce3013-f678-4c6a-935b-f4752ff8901b.xml"}, "meanAmount": 0.0, "other": {"anies": [{"value": "5.34834547E-8", "module": "A1", "scenario": "Standard scenario"}, {"value": "2.66210882E-8", "module": "A2", "scenario": "Standard scenario"}, {"value": "7.17501961E-8", "module": "A3", "scenario": "Standard scenario"}, {"value": "6.26224571E-8", "module": "A4", "scenario": "Standard scenario"}, {"value": "2.55785862E-8", "module": "A5", "scenario": "Standard scenario"}, {"value": "0.0", "module": "C1", "scenario": "Standard scenario"}, {"value": "8.4233807E-9", "module": "C2", "scenario": "Standard scenario"}, {"value": "0.0", "module": "C3", "scenario": "Standard scenario"}, {"value": "6.743736E-9", "module": "C4", "scenario": "Standard scenario"}, {"value": "-2.91396429E-8", "module": "D", "scenario": "Standard scenario"}, {"name": "referenceToUnitGroupDataSet", "value": {"shortDescription": [{"value": "disease incidence"}], "type": "unit group data set", "refObjectId": "3883559b-648f-4afc-8ba2-0bd24f3affa3", "uri": "../unitgroups/3883559b-648f-4afc-8ba2-0bd24f3affa3"}}]}}, {"referenceToLCIAMethodDataSet": {"shortDescription": [{"value": "Potenzielle Wirkung durch Exposition des Menschen mit U235 (IRP)", "lang": "de"}, {"value": "Potential Human exposure efficiency relative to U235 (IRP)", "lang": "en"}, {"value": "Exponeringseffektivitet relaterad till U235 (IR)", "lang": "sv"}], "type": "LCIA method data set", "refObjectId": "b5c632be-def3-11e6-bf01-fe55135034f3", "version": "01.00.013", "uri": "http://lca.jrc.ec.europa.eu/lcainfohub/datasets/elcd/lciamethods/a6f4cbc8-5388-44d6-9a67-53d05684f93e.xml"}, "meanAmount": 0.0, "other": {"anies": [{"value": "0.0385218327172722", "module": "A1", "scenario": "Standard scenario"}, {"value": "0.0186989215203058", "module": "A2", "scenario": "Standard scenario"}, {"value": "0.040263732400523", "module": "A3", "scenario": "Standard scenario"}, {"value": "0.0439866469973059", "module": "A4", "scenario": "Standard scenario"}, {"value": "0.010759397768385", "module": "A5", "scenario": "Standard scenario"}, {"value": "0.0", "module": "C1", "scenario": "Standard scenario"}, {"value": "0.0059166677691822", "module": "C2", "scenario": "Standard scenario"}, {"value": "0.0", "module": "C3", "scenario": "Standard scenario"}, {"value": "0.004190552", "module": "C4", "scenario": "Standard scenario"}, {"value": "-0.0025657304745329", "module": "D", "scenario": "Standard scenario"}, {"name": "referenceToUnitGroupDataSet", "value": {"shortDescription": [{"value": "kBq U235 eqv."}], "type": "unit group data set", "refObjectId": "456b05bf-1415-44a9-9993-02452f554c09", "uri": "../unitgroups/456b05bf-1415-44a9-9993-02452f554c09"}}]}}, {"referenceToLCIAMethodDataSet": {"shortDescription": [{"value": "Potenzielle Toxizitätsvergleichseinheit für Ökosysteme (ETP-fw)", "lang": "de"}, {"value": "Potential Comparative Toxic Unit for ecosystems (ETP-fw)", "lang": "en"}, {"value": "Ecotoxicitet (ETP-fw) ", "lang": "sv"}], "type": "LCIA method data set", "refObjectId": "ee1082d1-b0f7-43ca-a1f0-21e2a4a74511", "version": "01.00.004", "uri": "http://lca.jrc.ec.europa.eu/lcainfohub/datasets/elcd/lciamethods/ee1082d1-b0f7-43ca-a1f0-21e2a4a74511.xml"}, "meanAmount": 0.0, "other": {"anies": [{"value": "21.485774998588", "module": "A1", "scenario": "Standard scenario"}, {"value": "3.97966707234613", "module": "A2", "scenario": "Standard scenario"}, {"value": "20.1219560258195", "module": "A3", "scenario": "Standard scenario"}, {"value": "9.36162069496871", "module": "A4", "scenario": "Standard scenario"}, {"value": "8.99356368689789", "module": "A5", "scenario": "Standard scenario"}, {"value": "0.0", "module": "C1", "scenario": "Standard scenario"}, {"value": "1.25923668236459", "module": "C2", "scenario": "Standard scenario"}, {"value": "0.0", "module": "C3", "scenario": "Standard scenario"}, {"value": "0.662572062", "module": "C4", "scenario": "Standard scenario"}, {"value": "-19.7519508304061", "module": "D", "scenario": "Standard scenario"}, {"name": "referenceToUnitGroupDataSet", "value": {"shortDescription": [{"value": "CTUe"}], "type": "unit group data set", "refObjectId": "aa959ded-f1eb-4efb-9c5c-2d60be36b3e6", "uri": "../unitgroups/aa959ded-f1eb-4efb-9c5c-2d60be36b3e6"}}]}}, {"referenceToLCIAMethodDataSet": {"shortDescription": [{"value": "Potenzielle Toxizitätsvergleichseinheit für den Menschen - kanzerogene Wirkung (HTP-c)", "lang": "de"}, {"value": "Potential Comparative Toxic Unit for humans - cancer effects (HTP-c)", "lang": "en"}, {"value": "Humantoxicitet – cancer (HTP-c)", "lang": "sv"}], "type": "LCIA method data set", "refObjectId": "2299222a-bbd8-474f-9d4f-4dd1f18aea7c", "version": "01.00.005", "uri": "http://lca.jrc.ec.europa.eu/lcainfohub/datasets/elcd/lciamethods/2299222a-bbd8-474f-9d4f-4dd1f18aea7c.xml"}, "meanAmount": 0.0, "other": {"anies": [{"value": "6.66573E-10", "module": "A1", "scenario": "Standard scenario"}, {"value": "1.290782E-10", "module": "A2", "scenario": "Standard scenario"}, {"value": "1.5116021E-9", "module": "A3", "scenario": "Standard scenario"}, {"value": "3.036388E-10", "module": "A4", "scenario": "Standard scenario"}, {"value": "1.5848865E-9", "module": "A5", "scenario": "Standard scenario"}, {"value": "0.0", "module": "C1", "scenario": "Standard scenario"}, {"value": "4.08426E-11", "module": "C2", "scenario": "Standard scenario"}, {"value": "0.0", "module": "C3", "scenario": "Standard scenario"}, {"value": "1.5333E-11", "module": "C4", "scenario": "Standard scenario"}, {"value": "-2.602096E-10", "module": "D", "scenario": "Standard scenario"}, {"name": "referenceToUnitGroupDataSet", "value": {"shortDescription": [{"value": "CTUh"}], "type": "unit group data set", "refObjectId": "d4c9523e-2d7e-49fd-8469-998f547d3a70", "uri": "../unitgroups/d4c9523e-2d7e-49fd-8469-998f547d3a70"}}]}}, {"referenceToLCIAMethodDataSet": {"shortDescription": [{"value": "Potenzielle Toxizitätsvergleichseinheit für den Menschen - nicht kanzerogene Wirkung (HTP-nc)", "lang": "de"}, {"value": "Potential Comparative Toxic Unit for humans - non-cancer effects (HTP-nc)", "lang": "en"}, {"value": "Humantoxicitet – icke cancer (HTP-nc)", "lang": "sv"}], "type": "LCIA method data set", "refObjectId": "3af763a5-b7a1-48c9-9cee-1f223481fcef", "version": "01.00.004", "uri": "http://lca.jrc.ec.europa.eu/lcainfohub/datasets/elcd/lciamethods/3af763a5-b7a1-48c9-9cee-1f223481fcef.xml"}, "meanAmount": 0.0, "other": {"anies": [{"value": "2.46956763E-8", "module": "A1", "scenario": "Standard scenario"}, {"value": "4.3531578E-9", "module": "A2", "scenario": "Standard scenario"}, {"value": "1.58329764E-8", "module": "A3", "scenario": "Standard scenario"}, {"value": "1.02402063E-8", "module": "A4", "scenario": "Standard scenario"}, {"value": "1.78988011E-8", "module": "A5", "scenario": "Standard scenario"}, {"value": "0.0", "module": "C1", "scenario": "Standard scenario"}, {"value": "1.3774157E-9", "module": "C2", "scenario": "Standard scenario"}, {"value": "0.0", "module": "C3", "scenario": "Standard scenario"}, {"value": "4.710902E-10", "module": "C4", "scenario": "Standard scenario"}, {"value": "1.990852E-9", "module": "D", "scenario": "Standard scenario"}, {"name": "referenceToUnitGroupDataSet", "value": {"shortDescription": [{"value": "CTUh"}], "type": "unit group data set", "refObjectId": "d4c9523e-2d7e-49fd-8469-998f547d3a70", "uri": "../unitgroups/d4c9523e-2d7e-49fd-8469-998f547d3a70"}}]}}, {"referenceToLCIAMethodDataSet": {"shortDescription": [{"value": "Potenzieller Bodenqualitätsindex (SQP)", "lang": "de"}, {"value": "Potential Soil quality index (SQP)", "lang": "en"}, {"value": "Potentiell jordkvalitet index (SQP)", "lang": "sv"}], "type": "LCIA method data set", "refObjectId": "b2ad6890-c78d-11e6-9d9d-cec0c932ce01", "version": "01.00.014"}, "meanAmount": 0.0, "other": {"anies": [{"value": "4.40244766889304", "module": "A1", "scenario": "Standard scenario"}, {"value": "3.87042047376482", "module": "A2", "scenario": "Standard scenario"}, {"value": "232.176936913184", "module": "A3", "scenario": "Standard scenario"}, {"value": "9.10463306270157", "module": "A4", "scenario": "Standard scenario"}, {"value": "8.62252462263441", "module": "A5", "scenario": "Standard scenario"}, {"value": "0.0", "module": "C1", "scenario": "Standard scenario"}, {"value": "1.2246691364226", "module": "C2", "scenario": "Standard scenario"}, {"value": "0.0", "module": "C3", "scenario": "Standard scenario"}, {"value": "2.14206587199999", "module": "C4", "scenario": "Standard scenario"}, {"value": "-77.666036310767", "module": "D", "scenario": "Standard scenario"}, {"name": "referenceToUnitGroupDataSet", "value": {"shortDescription": [{"value": "dimensionless"}], "type": "unit group data set", "refObjectId": "f130951c-e67f-4f7f-8dd4-665de3974e18", "uri": "../unitgroups/f130951c-e67f-4f7f-8dd4-665de3974e18"}}]}}]}, "otherAttributes": {"{http://www.indata.network/EPD/2019}epd-version": "1.2", "{http://www.okworx.com/ILCD/Extensions/2018/Profile}profile": "EN_15804_A2"}, "version": "1.1"}