{"processInformation": {"dataSetInformation": {"UUID": "a76b254c-8958-4b45-8932-944097b77fbc", "name": {"baseName": [{"value": "EnkaSolutions and XeroFlor vegetation carriers (Freudenberg Performance Materials B.V.)", "lang": "en"}]}, "classificationInformation": {"classification": [{"class": [{"value": "Kunststoffe", "level": 0, "classId": "6"}, {"value": "Folien und Vliese", "level": 1, "classId": "6.6"}, {"value": "Technische Textilien", "level": 2, "classId": "6.6.07"}], "name": "OEKOBAU.DAT"}]}, "generalComment": [{"value": "The owner of this EPD shall be liable for the underlying information and evidence. The programme operator Kiwa-Ecobility Experts shall not be liable with respect to manufacturer data, life cycle assessment data and evidence.\r\nThis is a Cradle to gate with modules C1-C4 and module D EPD.\r\nNote: The EPD results have been calculated using the scaling method. The results table shown in this data set refers to the product XF 321 with the specific mass of 1.06 kg/m^2.\r\n", "lang": "en"}], "other": {"anies": [{}, {"scenario": [{"description": [{"value": "All datasets chosen for the LCA refer to Europe as the geographic reference.  A dataset for a non-specific truck was used for module A2. For the demolition (module C1), it is assumed that 0,001 liter diesel is used.  For the end-of-life, waste scenarios from the Dutch Environmental Database (Nationale Milieudatabase (NMD)) were used.", "lang": "en"}], "name": "Standard scenario", "default": true}]}, "<ns11:modules xmlns:ns11=\"http://openlca.org/epd_ilcd\" xmlns=\"http://lca.jrc.it/ILCD/Process\" xmlns:c=\"http://lca.jrc.it/ILCD/Contact\" xmlns:common=\"http://lca.jrc.it/ILCD/Common\" xmlns:epd=\"http://www.iai.kit.edu/EPD/2013\" xmlns:epd2=\"http://www.indata.network/EPD/2019\" xmlns:f=\"http://lca.jrc.it/ILCD/Flow\" xmlns:fp=\"http://lca.jrc.it/ILCD/FlowProperty\" xmlns:m=\"http://lca.jrc.it/ILCD/LCIAMethod\" xmlns:s=\"http://lca.jrc.it/ILCD/Source\" xmlns:u=\"http://lca.jrc.it/ILCD/UnitGroup\" name=\"A1\" scenario=\"Standard scenario\"/>", "<ns11:modules xmlns:ns11=\"http://openlca.org/epd_ilcd\" xmlns=\"http://lca.jrc.it/ILCD/Process\" xmlns:c=\"http://lca.jrc.it/ILCD/Contact\" xmlns:common=\"http://lca.jrc.it/ILCD/Common\" xmlns:epd=\"http://www.iai.kit.edu/EPD/2013\" xmlns:epd2=\"http://www.indata.network/EPD/2019\" xmlns:f=\"http://lca.jrc.it/ILCD/Flow\" xmlns:fp=\"http://lca.jrc.it/ILCD/FlowProperty\" xmlns:m=\"http://lca.jrc.it/ILCD/LCIAMethod\" xmlns:s=\"http://lca.jrc.it/ILCD/Source\" xmlns:u=\"http://lca.jrc.it/ILCD/UnitGroup\" name=\"A1-A3\" scenario=\"Standard scenario\"/>", "<ns11:modules xmlns:ns11=\"http://openlca.org/epd_ilcd\" xmlns=\"http://lca.jrc.it/ILCD/Process\" xmlns:c=\"http://lca.jrc.it/ILCD/Contact\" xmlns:common=\"http://lca.jrc.it/ILCD/Common\" xmlns:epd=\"http://www.iai.kit.edu/EPD/2013\" xmlns:epd2=\"http://www.indata.network/EPD/2019\" xmlns:f=\"http://lca.jrc.it/ILCD/Flow\" xmlns:fp=\"http://lca.jrc.it/ILCD/FlowProperty\" xmlns:m=\"http://lca.jrc.it/ILCD/LCIAMethod\" xmlns:s=\"http://lca.jrc.it/ILCD/Source\" xmlns:u=\"http://lca.jrc.it/ILCD/UnitGroup\" name=\"A2\" scenario=\"Standard scenario\"/>", "<ns11:modules xmlns:ns11=\"http://openlca.org/epd_ilcd\" xmlns=\"http://lca.jrc.it/ILCD/Process\" xmlns:c=\"http://lca.jrc.it/ILCD/Contact\" xmlns:common=\"http://lca.jrc.it/ILCD/Common\" xmlns:epd=\"http://www.iai.kit.edu/EPD/2013\" xmlns:epd2=\"http://www.indata.network/EPD/2019\" xmlns:f=\"http://lca.jrc.it/ILCD/Flow\" xmlns:fp=\"http://lca.jrc.it/ILCD/FlowProperty\" xmlns:m=\"http://lca.jrc.it/ILCD/LCIAMethod\" xmlns:s=\"http://lca.jrc.it/ILCD/Source\" xmlns:u=\"http://lca.jrc.it/ILCD/UnitGroup\" name=\"A3\" scenario=\"Standard scenario\"/>", "<ns11:modules xmlns:ns11=\"http://openlca.org/epd_ilcd\" xmlns=\"http://lca.jrc.it/ILCD/Process\" xmlns:c=\"http://lca.jrc.it/ILCD/Contact\" xmlns:common=\"http://lca.jrc.it/ILCD/Common\" xmlns:epd=\"http://www.iai.kit.edu/EPD/2013\" xmlns:epd2=\"http://www.indata.network/EPD/2019\" xmlns:f=\"http://lca.jrc.it/ILCD/Flow\" xmlns:fp=\"http://lca.jrc.it/ILCD/FlowProperty\" xmlns:m=\"http://lca.jrc.it/ILCD/LCIAMethod\" xmlns:s=\"http://lca.jrc.it/ILCD/Source\" xmlns:u=\"http://lca.jrc.it/ILCD/UnitGroup\" name=\"C1\" scenario=\"Standard scenario\"/>", "<ns11:modules xmlns:ns11=\"http://openlca.org/epd_ilcd\" xmlns=\"http://lca.jrc.it/ILCD/Process\" xmlns:c=\"http://lca.jrc.it/ILCD/Contact\" xmlns:common=\"http://lca.jrc.it/ILCD/Common\" xmlns:epd=\"http://www.iai.kit.edu/EPD/2013\" xmlns:epd2=\"http://www.indata.network/EPD/2019\" xmlns:f=\"http://lca.jrc.it/ILCD/Flow\" xmlns:fp=\"http://lca.jrc.it/ILCD/FlowProperty\" xmlns:m=\"http://lca.jrc.it/ILCD/LCIAMethod\" xmlns:s=\"http://lca.jrc.it/ILCD/Source\" xmlns:u=\"http://lca.jrc.it/ILCD/UnitGroup\" name=\"C2\" scenario=\"Standard scenario\"/>", "<ns11:modules xmlns:ns11=\"http://openlca.org/epd_ilcd\" xmlns=\"http://lca.jrc.it/ILCD/Process\" xmlns:c=\"http://lca.jrc.it/ILCD/Contact\" xmlns:common=\"http://lca.jrc.it/ILCD/Common\" xmlns:epd=\"http://www.iai.kit.edu/EPD/2013\" xmlns:epd2=\"http://www.indata.network/EPD/2019\" xmlns:f=\"http://lca.jrc.it/ILCD/Flow\" xmlns:fp=\"http://lca.jrc.it/ILCD/FlowProperty\" xmlns:m=\"http://lca.jrc.it/ILCD/LCIAMethod\" xmlns:s=\"http://lca.jrc.it/ILCD/Source\" xmlns:u=\"http://lca.jrc.it/ILCD/UnitGroup\" name=\"C3\" scenario=\"Standard scenario\"/>", "<ns11:modules xmlns:ns11=\"http://openlca.org/epd_ilcd\" xmlns=\"http://lca.jrc.it/ILCD/Process\" xmlns:c=\"http://lca.jrc.it/ILCD/Contact\" xmlns:common=\"http://lca.jrc.it/ILCD/Common\" xmlns:epd=\"http://www.iai.kit.edu/EPD/2013\" xmlns:epd2=\"http://www.indata.network/EPD/2019\" xmlns:f=\"http://lca.jrc.it/ILCD/Flow\" xmlns:fp=\"http://lca.jrc.it/ILCD/FlowProperty\" xmlns:m=\"http://lca.jrc.it/ILCD/LCIAMethod\" xmlns:s=\"http://lca.jrc.it/ILCD/Source\" xmlns:u=\"http://lca.jrc.it/ILCD/UnitGroup\" name=\"C4\" scenario=\"Standard scenario\"/>", "<ns11:modules xmlns:ns11=\"http://openlca.org/epd_ilcd\" xmlns=\"http://lca.jrc.it/ILCD/Process\" xmlns:c=\"http://lca.jrc.it/ILCD/Contact\" xmlns:common=\"http://lca.jrc.it/ILCD/Common\" xmlns:epd=\"http://www.iai.kit.edu/EPD/2013\" xmlns:epd2=\"http://www.indata.network/EPD/2019\" xmlns:f=\"http://lca.jrc.it/ILCD/Flow\" xmlns:fp=\"http://lca.jrc.it/ILCD/FlowProperty\" xmlns:m=\"http://lca.jrc.it/ILCD/LCIAMethod\" xmlns:s=\"http://lca.jrc.it/ILCD/Source\" xmlns:u=\"http://lca.jrc.it/ILCD/UnitGroup\" name=\"D\" scenario=\"Standard scenario\"/>", {}]}}, "quantitativeReference": {"referenceToReferenceFlow": [1], "type": "Reference flow(s)"}, "time": {"referenceYear": 2022, "dataSetValidUntil": 2029, "timeRepresentativenessDescription": [{"value": "All process-specific data were collected for the operating year 2022.", "lang": "en"}], "other": {"anies": [{"name": "publicationDateOfEPD", "value": 1731888000000}]}}, "geography": {"locationOfOperationSupplyOrProduction": {"descriptionOfRestrictions": [{"value": "The data are representative for the European Union.", "lang": "en"}], "location": "EU-27"}}, "technology": {"technologyDescriptionAndIncludedProcesses": [{"value": "Enka vegetation carriers are synthetic and durable mats which consist out of two components: a lightweight, flexible and very open three-dimensional matting made of entangled polyamide filaments on the top surface. And a nonwoven filter fabric underneath. Both components are filmy connected. The Enka vegetation carrier is delivered in easy-to-handle 3.2 feet or 1 m wide rolls. The vegetation carrier product range consist of a polyamide pyramid structure with on one side a thermally bonded nonwoven. The polyamide structure is produced at the Obernburg am Main site through a monofilament extrusion process. The polyamide chips are delivered by truck from Luxembourg. The thermally bonded nonwoven is delivered from the Netherlands. After coupling the structure and the thermally bonded nonwoven at the Obernburg am Main site the rolls winded on a tube, strapped and covered in black PE foil. The final roll length can vary between 50 and 100m. Depending on the customers request or optimal loading of a truck. ", "lang": "en"}], "technologicalApplicability": [{"value": "The vegetation carrier is used to create pre-vegetated matts or erosion prevention by reinforcing root structures. Application areas where this can be applied green roofs, tram ways, landscaping, dykes or slopes. The thickness of the matt guarantees a minimal substrate thickness and minimal waste while harvesting and installing pre-vegetated matts. The geotextile will be penetrated by the roots which allows the fully grown and rooted matt to behave like a blanket. The geotextile makes sure the soil stays separated from the subfloor. ", "lang": "en"}], "referenceToTechnologyFlowDiagrammOrPicture": [{"shortDescription": [{"value": "Flow chart EnkaSolutions and XeroFlor vegetation carriers ", "lang": "en"}], "type": "source data set", "refObjectId": "4e44ed55-e96c-4f7f-9deb-3290108fbe0b", "version": "00.00.001"}]}}, "modellingAndValidation": {"LCIMethodAndAllocation": {"typeOfDataSet": "EPD", "other": {"anies": [{"name": "subType", "value": "specific dataset"}]}}, "dataSourcesTreatmentAndRepresentativeness": {"referenceToDataSource": [{"shortDescription": [{"value": "ecoinvent 3.6 database", "lang": "en"}], "type": "source data set", "refObjectId": "766b9973-5ee8-48a2-8098-72c8e20b369f", "version": "00.00.001"}, {"shortDescription": [{"value": "ecoinvent database (general)", "lang": "en"}], "type": "source data set", "refObjectId": "b497a91f-e14b-4b69-8f28-f50eb1576766", "version": "00.03.002"}], "useAdviceForDataSet": [{"value": "The vegetation carrier is used to create pre-vegetated matts or erosion prevention by reinforcing root structures. Application areas where this can be applied green roofs, tram ways, landscaping, dykes or slopes. The thickness of the matt guarantees a minimal substrate thickness and minimal waste while harvesting and installing pre-vegetated matts. The geotextile will be penetrated by the roots which allows the fully grown and rooted matt to behave like a blanket. The geotextile makes sure the soil stays separated from the subfloor. ", "lang": "en"}], "other": {"anies": [{"name": "referenceToOriginalEPD", "value": {"shortDescription": {"value": "EnkaSolutions and XeroFlor vegetation carriers EPD", "defaultValue": "EnkaSolutions and XeroFlor vegetation carriers EPD", "lstrings": [{"lang": "en", "value": "EnkaSolutions and XeroFlor vegetation carriers EPD"}]}, "version": {"version": 1, "majorVersion": 0, "minorVersion": 0, "subMinorVersion": 1, "zero": false, "versionString": "00.00.001"}, "type": "source data set", "uuid": {"uuid": "ee1747e9-6ed3-4303-82ae-e0453f2ae5ec"}, "refObjectId": "ee1747e9-6ed3-4303-82ae-e0453f2ae5ec", "versionAsString": "00.00.001", "resourceURLs": ["https://oekobaudat.de/OEKOBAU.DAT/resource/sources/ee1747e9-6ed3-4303-82ae-e0453f2ae5ec/EPD-Kiwa-EE-172731-EN.pdf?version=00.00.001"]}}]}}, "validation": {"review": [{"reviewDetails": [{"value": "The independent verification is in accordance with the ISO 14025:2011.", "lang": "en"}], "referenceToNameOfReviewerAndInstitution": [{"shortDescription": [{"value": "Lucas Pedro Berman, Senda", "lang": "en"}], "type": "contact data set", "refObjectId": "2294137c-5a52-4a75-965f-770e74b24b10", "version": "00.00.002"}], "type": "Independent external review"}]}, "complianceDeclarations": {"compliance": [{"referenceToComplianceSystem": {"shortDescription": [{"value": "ISO 14025", "lang": "en"}], "type": "source data set", "refObjectId": "4f2eb655-6e44-4874-a95a-e28f5442cd4d", "version": "00.00.001"}}, {"referenceToComplianceSystem": {"shortDescription": [{"value": "EN 15804+A2 (EF 3.1)", "lang": "de"}, {"value": "EN 15804+A2 (EF 3.1)", "lang": "en"}], "type": "source data set", "refObjectId": "d4aa3ec7-b1d7-4a4a-a6cb-37af88dcc902", "version": "00.01.000"}}]}}, "administrativeInformation": {"commissionerAndGoal": {"referenceToCommissioner": [{"shortDescription": [{"value": "Freudenberg Performance Materials B.V.", "lang": "en"}], "type": "contact data set", "refObjectId": "adc064d8-4c1f-4127-8ae9-cae8ea04141f", "version": "00.00.001"}]}, "dataGenerator": {"referenceToPersonOrEntityGeneratingTheDataSet": [{"shortDescription": [{"value": "Kiwa GmbH (Berlin)", "lang": "en"}], "type": "contact data set", "refObjectId": "3ea4a87a-3f88-4633-b7e7-1bbdd272be43", "version": "00.00.002"}]}, "dataEntryBy": {"timeStamp": 1740393371863, "referenceToDataSetFormat": [{"shortDescription": [{"value": "EPD Data Format Extensions v1.2", "lang": "en"}, {"value": "EPD-Datenformaterweiterungen v1.2", "lang": "de"}], "type": "source data set", "refObjectId": "a29449fd-aa2f-4de8-b5d7-4b06b43c6fde", "version": "00.01.000"}, {"shortDescription": [{"value": "ILCD format", "lang": "en"}], "type": "source data set", "refObjectId": "a97a0155-0234-4b87-b4ce-a45da52f2a40", "version": "01.00.000", "uri": "http://lca.jrc.ec.europa.eu/lcainfohub/sample_data/ilcd/sources/ILCD_Format_a97a0155-0234-4b87-b4ce-a45da52f2a40_01.00.000.xml"}], "referenceToPersonOrEntityEnteringTheData": {"shortDescription": [{"value": "Kiwa GmbH (Berlin)", "lang": "en"}], "type": "contact data set", "refObjectId": "3ea4a87a-3f88-4633-b7e7-1bbdd272be43", "version": "00.00.002"}}, "publicationAndOwnership": {"dataSetVersion": "00.00.008", "referenceToRegistrationAuthority": {"shortDescription": [{"value": "Kiwa-Ecobility Experts, Kiwa GmbH (Berlin)", "lang": "en"}], "type": "contact data set", "refObjectId": "eb52a9a8-9d0f-40ce-a5c9-7b78f5615e5a", "version": "00.00.002"}, "registrationNumber": "EPD-Kiwa-EE-172731-EN", "referenceToOwnershipOfDataSet": {"shortDescription": [{"value": "Freudenberg Performance Materials B.V.", "lang": "en"}], "type": "contact data set", "refObjectId": "adc064d8-4c1f-4127-8ae9-cae8ea04141f", "version": "00.00.001"}, "copyright": true, "licenseType": "Free of charge for all users and uses", "accessRestrictions": [{"value": "None.", "lang": "en"}], "other": {"anies": [{"name": "referenceToPublisher", "value": {"shortDescription": [{"value": "Kiwa-Ecobility Experts, Kiwa GmbH (Berlin)", "lang": "en"}], "type": "contact data set", "refObjectId": "eb52a9a8-9d0f-40ce-a5c9-7b78f5615e5a", "version": "00.00.002"}}]}}}, "exchanges": {"exchange": [{"dataSetInternalID": 1, "referenceToFlowDataSet": {"shortDescription": [{"value": "EnkaSolutions and XeroFlor vegetation carriers (Freudenberg Performance Materials B.V.)", "lang": "en"}], "type": "flow data set", "refObjectId": "844d3135-e490-4b3c-8092-e7d41a89c40d", "version": "00.00.005"}, "meanAmount": 1.0, "resultingAmount": 1.0, "referenceFlow": true, "resultingflowAmount": 1.0, "flowProperties": [{"name": [{"lang": "de", "value": "Fläche"}, {"lang": "en", "value": "Area"}], "uuid": "93a60a56-a3c8-19da-a746-0800200c9a66", "referenceFlowProperty": true, "meanValue": 1.0, "referenceUnit": "qm", "unitGroupUUID": "c20a03d7-bd90-4569-bc94-66cfd364dfc8"}], "materialProperties": [{"name": "grammage", "value": "1.06", "unit": "kg/m^2", "unitDescription": "kilograms per square meter"}, {"name": "layer thickness", "value": "0.016", "unit": "m", "unitDescription": "meters"}], "typeOfFlow": "Product flow", "classification": {"classHierarchy": "Kunststoffe / Folien und Vliese / Technische Textilien", "name": "OEKOBAU.DAT"}}, {"dataSetInternalID": 2, "referenceToFlowDataSet": {"shortDescription": [{"value": "Components for re-use (CRU)", "lang": "en"}, {"value": "Komponenten für die Wiederverwendung (CRU)", "lang": "de"}, {"value": "Componentes para su reutilización (CRU)", "lang": "es"}], "type": "flow data set", "refObjectId": "a2b32f97-3fc7-4af2-b209-525bc6426f33", "version": "30.00.000", "uri": "../flows/a2b32f97-3fc7-4af2-b209-525bc6426f33.xml"}, "exchange direction": "OUTPUT", "meanAmount": 0.0, "other": {"anies": [{"value": "0.0", "module": "A1", "scenario": "Standard scenario"}, {"value": "0.0", "module": "A2", "scenario": "Standard scenario"}, {"value": "0.0", "module": "A3", "scenario": "Standard scenario"}, {"value": "0.0", "module": "A1-A3", "scenario": "Standard scenario"}, {"value": "0.0", "module": "C1", "scenario": "Standard scenario"}, {"value": "0.0", "module": "C2", "scenario": "Standard scenario"}, {"value": "0.0", "module": "C3", "scenario": "Standard scenario"}, {"value": "0.0", "module": "C4", "scenario": "Standard scenario"}, {"value": "0.0", "module": "D", "scenario": "Standard scenario"}, {"name": "referenceToUnitGroupDataSet", "value": {"shortDescription": [{"value": "kg", "lang": "en"}], "type": "unit group data set", "refObjectId": "ad38d542-3fe9-439d-9b95-2f5f7752acaf", "version": "30.00.000", "uri": "../unitgroups/ad38d542-3fe9-439d-9b95-2f5f7752acaf.xml"}}]}, "flowProperties": [], "typeOfFlow": "Other flow", "classification": {"classHierarchy": "Größen / Umweltliche Größen / EPD EN 15804 / LCI Indikatoren", "name": "GaBiCategories"}}, {"dataSetInternalID": 3, "referenceToFlowDataSet": {"shortDescription": [{"value": "Exported electrical energy (EEE)", "lang": "en"}, {"value": "Exportierte elektrische Energie (EEE)", "lang": "de"}, {"value": "Energía exportada electrica (EEE)", "lang": "es"}], "type": "flow data set", "refObjectId": "4da0c987-2b76-40d6-9e9e-82a017aaaf29", "version": "30.00.000", "uri": "../flows/4da0c987-2b76-40d6-9e9e-82a017aaaf29.xml"}, "exchange direction": "OUTPUT", "meanAmount": 0.0, "other": {"anies": [{"value": "0.0", "module": "A1", "scenario": "Standard scenario"}, {"value": "0.0", "module": "A2", "scenario": "Standard scenario"}, {"value": "-0.07142353504668", "module": "A3", "scenario": "Standard scenario"}, {"value": "-0.07142353504668", "module": "A1-A3", "scenario": "Standard scenario"}, {"value": "0.0", "module": "C1", "scenario": "Standard scenario"}, {"value": "0.0", "module": "C2", "scenario": "Standard scenario"}, {"value": "0.0", "module": "C3", "scenario": "Standard scenario"}, {"value": "0.0", "module": "C4", "scenario": "Standard scenario"}, {"value": "-2.6573169744000014", "module": "D", "scenario": "Standard scenario"}, {"name": "referenceToUnitGroupDataSet", "value": {"shortDescription": [{"value": "MJ", "lang": "en"}], "type": "unit group data set", "refObjectId": "93a60a57-a3c8-11da-a746-0800200c9a66", "version": "03.00.000", "uri": "../unitgroups/93a60a57-a3c8-11da-a746-0800200c9a66.xml"}}]}, "flowProperties": [], "typeOfFlow": "Other flow", "classification": {"classHierarchy": "Größen / Umweltliche Größen / EPD EN 15804 / LCI Indikatoren", "name": "GaBiCategories"}}, {"dataSetInternalID": 4, "referenceToFlowDataSet": {"shortDescription": [{"value": "Exported thermal energy (EET)", "lang": "en"}, {"value": "Exportierte thermische Energie (EET)", "lang": "de"}, {"value": "Energía exportada termal (EET)", "lang": "es"}], "type": "flow data set", "refObjectId": "98daf38a-7a79-46d3-9a37-2b7bd0955810", "version": "30.00.000", "uri": "../flows/98daf38a-7a79-46d3-9a37-2b7bd0955810.xml"}, "exchange direction": "OUTPUT", "meanAmount": 0.0, "other": {"anies": [{"value": "0.0", "module": "A1", "scenario": "Standard scenario"}, {"value": "0.0", "module": "A2", "scenario": "Standard scenario"}, {"value": "-0.12300719924706002", "module": "A3", "scenario": "Standard scenario"}, {"value": "-0.12300719924706002", "module": "A1-A3", "scenario": "Standard scenario"}, {"value": "0.0", "module": "C1", "scenario": "Standard scenario"}, {"value": "0.0", "module": "C2", "scenario": "Standard scenario"}, {"value": "0.0", "module": "C3", "scenario": "Standard scenario"}, {"value": "0.0", "module": "C4", "scenario": "Standard scenario"}, {"value": "-4.5764903448", "module": "D", "scenario": "Standard scenario"}, {"name": "referenceToUnitGroupDataSet", "value": {"shortDescription": [{"value": "MJ", "lang": "en"}], "type": "unit group data set", "refObjectId": "93a60a57-a3c8-11da-a746-0800200c9a66", "version": "03.00.000", "uri": "../unitgroups/93a60a57-a3c8-11da-a746-0800200c9a66.xml"}}]}, "flowProperties": [], "typeOfFlow": "Other flow", "classification": {"classHierarchy": "Größen / Umweltliche Größen / EPD EN 15804 / LCI Indikatoren", "name": "GaBiCategories"}}, {"dataSetInternalID": 5, "referenceToFlowDataSet": {"shortDescription": [{"value": "Use of net fresh water (FW)", "lang": "en"}, {"value": "Einsatz von Süßwasserressourcen (FW)", "lang": "de"}, {"value": "Uso neto de recursos de agua dulce (FW)", "lang": "es"}], "type": "flow data set", "refObjectId": "3cf952c8-f3a4-461d-8c96-96456ca62246", "version": "30.00.000", "uri": "../flows/3cf952c8-f3a4-461d-8c96-96456ca62246.xml"}, "exchange direction": "INPUT", "meanAmount": 0.0, "other": {"anies": [{"value": "0.061489352836122", "module": "A1", "scenario": "Standard scenario"}, {"value": "1.44685937818918E-4", "module": "A2", "scenario": "Standard scenario"}, {"value": "0.01712701355530507", "module": "A3", "scenario": "Standard scenario"}, {"value": "0.07876105232924599", "module": "A1-A3", "scenario": "Standard scenario"}, {"value": "2.3228564365E-6", "module": "C1", "scenario": "Standard scenario"}, {"value": "3.7574978990776E-5", "module": "C2", "scenario": "Standard scenario"}, {"value": "0.0033618989568", "module": "C3", "scenario": "Standard scenario"}, {"value": "5.6940972800000005E-5", "module": "C4", "scenario": "Standard scenario"}, {"value": "-5.930588459856001E-4", "module": "D", "scenario": "Standard scenario"}, {"name": "referenceToUnitGroupDataSet", "value": {"shortDescription": [{"value": "m3", "lang": "en"}], "type": "unit group data set", "refObjectId": "cd950537-0a98-4044-9ba7-9f9a68d0a504", "version": "30.00.000", "uri": "../unitgroups/cd950537-0a98-4044-9ba7-9f9a68d0a504.xml"}}]}, "flowProperties": [], "typeOfFlow": "Other flow", "classification": {"classHierarchy": "Größen / Umweltliche Größen / EPD EN 15804 / LCI Indikatoren", "name": "GaBiCategories"}}, {"dataSetInternalID": 6, "referenceToFlowDataSet": {"shortDescription": [{"value": "Hazardous waste disposed (HWD)", "lang": "en"}, {"value": "Gefährlicher Abfall zur Deponie (HWD)", "lang": "de"}, {"value": "Residuos peligrosos eliminados (HWD)", "lang": "es"}], "type": "flow data set", "refObjectId": "430f9e0f-59b2-46a0-8e0d-55e0e84948fc", "version": "30.00.000", "uri": "../flows/430f9e0f-59b2-46a0-8e0d-55e0e84948fc.xml"}, "exchange direction": "OUTPUT", "meanAmount": 0.0, "other": {"anies": [{"value": "4.843517109583E-5", "module": "A1", "scenario": "Standard scenario"}, {"value": "3.0099474233700005E-6", "module": "A2", "scenario": "Standard scenario"}, {"value": "5.132385400391E-5", "module": "A3", "scenario": "Standard scenario"}, {"value": "1.0276897252310999E-4", "module": "A1-A3", "scenario": "Standard scenario"}, {"value": "1.228900316E-7", "module": "C1", "scenario": "Standard scenario"}, {"value": "7.816841975740001E-7", "module": "C2", "scenario": "Standard scenario"}, {"value": "3.091699968E-6", "module": "C3", "scenario": "Standard scenario"}, {"value": "8.27051392E-8", "module": "C4", "scenario": "Standard scenario"}, {"value": "-1.3020181611508002E-5", "module": "D", "scenario": "Standard scenario"}, {"name": "referenceToUnitGroupDataSet", "value": {"shortDescription": [{"value": "kg", "lang": "en"}], "type": "unit group data set", "refObjectId": "ad38d542-3fe9-439d-9b95-2f5f7752acaf", "version": "30.00.000", "uri": "../unitgroups/ad38d542-3fe9-439d-9b95-2f5f7752acaf.xml"}}]}, "flowProperties": [], "typeOfFlow": "Other flow", "classification": {"classHierarchy": "Größen / Umweltliche Größen / EPD EN 15804 / LCI Indikatoren", "name": "GaBiCategories"}}, {"dataSetInternalID": 7, "referenceToFlowDataSet": {"shortDescription": [{"value": "Materials for energy recovery (MER)", "lang": "en"}, {"value": "Stoffe für die Energierückgewinnung (MER)", "lang": "de"}, {"value": "Materiales para valorización energética (recuperación de energía) (MER)", "lang": "es"}], "type": "flow data set", "refObjectId": "59a9181c-3aaf-46ee-8b13-2b3723b6e447", "version": "30.00.000", "uri": "../flows/59a9181c-3aaf-46ee-8b13-2b3723b6e447.xml"}, "exchange direction": "OUTPUT", "meanAmount": 0.0, "other": {"anies": [{"value": "0.0", "module": "A1", "scenario": "Standard scenario"}, {"value": "0.0", "module": "A2", "scenario": "Standard scenario"}, {"value": "0.0", "module": "A3", "scenario": "Standard scenario"}, {"value": "0.0", "module": "A1-A3", "scenario": "Standard scenario"}, {"value": "0.0", "module": "C1", "scenario": "Standard scenario"}, {"value": "0.0", "module": "C2", "scenario": "Standard scenario"}, {"value": "0.0", "module": "C3", "scenario": "Standard scenario"}, {"value": "0.0", "module": "C4", "scenario": "Standard scenario"}, {"value": "0.0", "module": "D", "scenario": "Standard scenario"}, {"name": "referenceToUnitGroupDataSet", "value": {"shortDescription": [{"value": "kg", "lang": "en"}], "type": "unit group data set", "refObjectId": "ad38d542-3fe9-439d-9b95-2f5f7752acaf", "version": "30.00.000", "uri": "../unitgroups/ad38d542-3fe9-439d-9b95-2f5f7752acaf.xml"}}]}, "flowProperties": [], "typeOfFlow": "Other flow", "classification": {"classHierarchy": "Größen / Umweltliche Größen / EPD EN 15804 / LCI Indikatoren", "name": "GaBiCategories"}}, {"dataSetInternalID": 8, "referenceToFlowDataSet": {"shortDescription": [{"value": "Materials for recycling (MFR)", "lang": "en"}, {"value": "Stoffe zum Recycling (MFR)", "lang": "de"}, {"value": "Materiales para el reciclaje (MFR)", "lang": "es"}], "type": "flow data set", "refObjectId": "d7fe48a5-4103-49c8-9aae-b0b5dfdbd6ae", "version": "30.00.000", "uri": "../flows/d7fe48a5-4103-49c8-9aae-b0b5dfdbd6ae.xml"}, "exchange direction": "OUTPUT", "meanAmount": 0.0, "other": {"anies": [{"value": "0.0", "module": "A1", "scenario": "Standard scenario"}, {"value": "0.0", "module": "A2", "scenario": "Standard scenario"}, {"value": "0.00130534885", "module": "A3", "scenario": "Standard scenario"}, {"value": "0.00130534885", "module": "A1-A3", "scenario": "Standard scenario"}, {"value": "0.0", "module": "C1", "scenario": "Standard scenario"}, {"value": "0.0", "module": "C2", "scenario": "Standard scenario"}, {"value": "0.0", "module": "C3", "scenario": "Standard scenario"}, {"value": "0.0", "module": "C4", "scenario": "Standard scenario"}, {"value": "0.0", "module": "D", "scenario": "Standard scenario"}, {"name": "referenceToUnitGroupDataSet", "value": {"shortDescription": [{"value": "kg", "lang": "en"}], "type": "unit group data set", "refObjectId": "ad38d542-3fe9-439d-9b95-2f5f7752acaf", "version": "30.00.000", "uri": "../unitgroups/ad38d542-3fe9-439d-9b95-2f5f7752acaf.xml"}}]}, "flowProperties": [], "typeOfFlow": "Other flow", "classification": {"classHierarchy": "Größen / Umweltliche Größen / EPD EN 15804 / LCI Indikatoren", "name": "GaBiCategories"}}, {"dataSetInternalID": 9, "referenceToFlowDataSet": {"shortDescription": [{"value": "Non-hazardous waste disposed (NHWD)", "lang": "en"}, {"value": "Entsorgter nicht gefährlicher Abfall (NHWD)", "lang": "de"}, {"value": "Residuos no peligrosos eliminados (NHWD)", "lang": "es"}], "type": "flow data set", "refObjectId": "b29ef66b-e286-4afa-949f-62f1a7b4d7fa", "version": "30.00.000", "uri": "../flows/b29ef66b-e286-4afa-949f-62f1a7b4d7fa.xml"}, "exchange direction": "OUTPUT", "meanAmount": 0.0, "other": {"anies": [{"value": "0.1506639074743", "module": "A1", "scenario": "Standard scenario"}, {"value": "0.0753449987451481", "module": "A2", "scenario": "Standard scenario"}, {"value": "0.014142580182971928", "module": "A3", "scenario": "Standard scenario"}, {"value": "0.24015148640242004", "module": "A1-A3", "scenario": "Standard scenario"}, {"value": "5.3419345853E-5", "module": "C1", "scenario": "Standard scenario"}, {"value": "0.019567117493135576", "module": "C2", "scenario": "Standard scenario"}, {"value": "0.0337688114432", "module": "C3", "scenario": "Standard scenario"}, {"value": "0.21702976005760002", "module": "C4", "scenario": "Standard scenario"}, {"value": "-0.004133224208202199", "module": "D", "scenario": "Standard scenario"}, {"name": "referenceToUnitGroupDataSet", "value": {"shortDescription": [{"value": "kg", "lang": "en"}], "type": "unit group data set", "refObjectId": "ad38d542-3fe9-439d-9b95-2f5f7752acaf", "version": "30.00.000", "uri": "../unitgroups/ad38d542-3fe9-439d-9b95-2f5f7752acaf.xml"}}]}, "flowProperties": [], "typeOfFlow": "Other flow", "classification": {"classHierarchy": "Größen / Umweltliche Größen / EPD EN 15804 / LCI Indikatoren", "name": "GaBiCategories"}}, {"dataSetInternalID": 10, "referenceToFlowDataSet": {"shortDescription": [{"value": "Use of non renewable secondary fuels (NRSF)", "lang": "en"}, {"value": "Nicht erneuerbare Sekundärbrennstoffe (NRSF)", "lang": "de"}, {"value": "Uso de combustibles secundarios no renovables (NRSF)", "lang": "es"}], "type": "flow data set", "refObjectId": "89def144-d39a-4287-b86f-efde453ddcb2", "version": "30.00.000", "uri": "../flows/89def144-d39a-4287-b86f-efde453ddcb2.xml"}, "exchange direction": "INPUT", "meanAmount": 0.0, "other": {"anies": [{"value": "0.0", "module": "A1", "scenario": "Standard scenario"}, {"value": "0.0", "module": "A2", "scenario": "Standard scenario"}, {"value": "0.0", "module": "A3", "scenario": "Standard scenario"}, {"value": "0.0", "module": "A1-A3", "scenario": "Standard scenario"}, {"value": "0.0", "module": "C1", "scenario": "Standard scenario"}, {"value": "0.0", "module": "C2", "scenario": "Standard scenario"}, {"value": "0.0", "module": "C3", "scenario": "Standard scenario"}, {"value": "0.0", "module": "C4", "scenario": "Standard scenario"}, {"value": "0.0", "module": "D", "scenario": "Standard scenario"}, {"name": "referenceToUnitGroupDataSet", "value": {"shortDescription": [{"value": "MJ", "lang": "en"}], "type": "unit group data set", "refObjectId": "93a60a57-a3c8-11da-a746-0800200c9a66", "version": "03.00.000", "uri": "../unitgroups/93a60a57-a3c8-11da-a746-0800200c9a66.xml"}}]}, "flowProperties": [], "typeOfFlow": "Other flow", "classification": {"classHierarchy": "Größen / Umweltliche Größen / EPD EN 15804 / LCI Indikatoren", "name": "GaBiCategories"}}, {"dataSetInternalID": 11, "referenceToFlowDataSet": {"shortDescription": [{"value": "Use of non renewable primary energy (PENRE)", "lang": "en"}, {"value": "Nicht-erneuerbare Primärenergie als Energieträger (PENRE)", "lang": "de"}, {"value": "Uso de energía primaria no renovable, excluyendo los recursos de energía primaria no renovable utilizada como materia prima (PENRE)", "lang": "es"}], "type": "flow data set", "refObjectId": "ac857178-2b45-46ec-892a-a9a4332f0372", "version": "38.00.000", "uri": "../flows/ac857178-2b45-46ec-892a-a9a4332f0372.xml"}, "exchange direction": "INPUT", "meanAmount": 0.0, "other": {"anies": [{"value": "112.42278834495188", "module": "A1", "scenario": "Standard scenario"}, {"value": "1.261102930120794", "module": "A2", "scenario": "Standard scenario"}, {"value": "3.925095199022327", "module": "A3", "scenario": "Standard scenario"}, {"value": "117.608986474095", "module": "A1-A3", "scenario": "Standard scenario"}, {"value": "0.0479144135182203", "module": "C1", "scenario": "Standard scenario"}, {"value": "0.32750878778400816", "module": "C2", "scenario": "Standard scenario"}, {"value": "1.6852129066751893", "module": "C3", "scenario": "Standard scenario"}, {"value": "0.0579739210176", "module": "C4", "scenario": "Standard scenario"}, {"value": "-11.412037426428139", "module": "D", "scenario": "Standard scenario"}, {"name": "referenceToUnitGroupDataSet", "value": {"shortDescription": [{"value": "MJ", "lang": "en"}], "type": "unit group data set", "refObjectId": "93a60a57-a3c8-11da-a746-0800200c9a66", "version": "03.00.000", "uri": "../unitgroups/93a60a57-a3c8-11da-a746-0800200c9a66.xml"}}]}, "flowProperties": [], "typeOfFlow": "Other flow", "classification": {"classHierarchy": "Quantities", "name": "GaBiCategories"}}, {"dataSetInternalID": 12, "referenceToFlowDataSet": {"shortDescription": [{"value": "Use of non renewable primary energy resources used as raw materials (PENRM)", "lang": "en"}, {"value": "Nicht-erneuerbare Primärenergie zur stofflichen Nutzung (PENRM)", "lang": "de"}, {"value": "Uso de la energía primaria no renovable utilizada como materia prima (PENRM)", "lang": "es"}], "type": "flow data set", "refObjectId": "1421caa0-679d-4bf4-b282-0eb850ccae27", "version": "38.00.000", "uri": "../flows/1421caa0-679d-4bf4-b282-0eb850ccae27.xml"}, "exchange direction": "INPUT", "meanAmount": 0.0, "other": {"anies": [{"value": "0.1796481", "module": "A1", "scenario": "Standard scenario"}, {"value": "0.0", "module": "A2", "scenario": "Standard scenario"}, {"value": "-0.045395431716115", "module": "A3", "scenario": "Standard scenario"}, {"value": "0.134252668283885", "module": "A1-A3", "scenario": "Standard scenario"}, {"value": "0.0", "module": "C1", "scenario": "Standard scenario"}, {"value": "0.0", "module": "C2", "scenario": "Standard scenario"}, {"value": "0.0", "module": "C3", "scenario": "Standard scenario"}, {"value": "0.0", "module": "C4", "scenario": "Standard scenario"}, {"value": "0.0", "module": "D", "scenario": "Standard scenario"}, {"name": "referenceToUnitGroupDataSet", "value": {"shortDescription": [{"value": "MJ", "lang": "en"}], "type": "unit group data set", "refObjectId": "93a60a57-a3c8-11da-a746-0800200c9a66", "version": "03.00.000", "uri": "../unitgroups/93a60a57-a3c8-11da-a746-0800200c9a66.xml"}}]}, "flowProperties": [], "typeOfFlow": "Other flow", "classification": {"classHierarchy": "Quantities", "name": "GaBiCategories"}}, {"dataSetInternalID": 13, "referenceToFlowDataSet": {"shortDescription": [{"value": "Total use of non-renewable primary energy resources (PENRT)", "lang": "en"}, {"value": "Total nicht erneuerbare Primärenergie (PENRT)", "lang": "de"}, {"value": "Uso total de la energía primaria no renovable (energía primaria y recursos de energía primaria renovable utilizada como materia prima) (PENRT)", "lang": "es"}], "type": "flow data set", "refObjectId": "06159210-646b-4c8d-8583-da9b3b95a6c1", "version": "30.00.000", "uri": "../flows/06159210-646b-4c8d-8583-da9b3b95a6c1.xml"}, "exchange direction": "INPUT", "meanAmount": 0.0, "other": {"anies": [{"value": "112.60243644495189", "module": "A1", "scenario": "Standard scenario"}, {"value": "1.261102930120794", "module": "A2", "scenario": "Standard scenario"}, {"value": "3.8796997673062066", "module": "A3", "scenario": "Standard scenario"}, {"value": "117.7432391423789", "module": "A1-A3", "scenario": "Standard scenario"}, {"value": "0.0479144135182203", "module": "C1", "scenario": "Standard scenario"}, {"value": "0.32750878778400816", "module": "C2", "scenario": "Standard scenario"}, {"value": "1.6852129066751893", "module": "C3", "scenario": "Standard scenario"}, {"value": "0.0579739210176", "module": "C4", "scenario": "Standard scenario"}, {"value": "-11.412037426428139", "module": "D", "scenario": "Standard scenario"}, {"name": "referenceToUnitGroupDataSet", "value": {"shortDescription": [{"value": "MJ", "lang": "en"}], "type": "unit group data set", "refObjectId": "93a60a57-a3c8-11da-a746-0800200c9a66", "version": "03.00.000", "uri": "../unitgroups/93a60a57-a3c8-11da-a746-0800200c9a66.xml"}}]}, "flowProperties": [], "typeOfFlow": "Other flow", "classification": {"classHierarchy": "Größen / Umweltliche Größen / EPD EN 15804 / LCI Indikatoren", "name": "GaBiCategories"}}, {"dataSetInternalID": 14, "referenceToFlowDataSet": {"shortDescription": [{"value": "Use of renewable primary energy (PERE)", "lang": "en"}, {"value": "Erneuerbare Primärenergie als Energieträger (PERE)", "lang": "de"}, {"value": "Uso de energía primaria renovable excluyendo los recursos de energía primaria renovable utilizada como materia prima (PERE)", "lang": "es"}], "type": "flow data set", "refObjectId": "20f32be5-0398-4288-9b6d-accddd195317", "version": "38.00.000", "uri": "../flows/20f32be5-0398-4288-9b6d-accddd195317.xml"}, "exchange direction": "INPUT", "meanAmount": 0.0, "other": {"anies": [{"value": "-17.243935834360904", "module": "A1", "scenario": "Standard scenario"}, {"value": "0.014870255268576112", "module": "A2", "scenario": "Standard scenario"}, {"value": "-0.03195819129662625", "module": "A3", "scenario": "Standard scenario"}, {"value": "-17.261023770388956", "module": "A1-A3", "scenario": "Standard scenario"}, {"value": "2.440438130167E-4", "module": "C1", "scenario": "Standard scenario"}, {"value": "0.0038618095008182245", "module": "C2", "scenario": "Standard scenario"}, {"value": "0.172212884352", "module": "C3", "scenario": "Standard scenario"}, {"value": "9.859665024E-4", "module": "C4", "scenario": "Standard scenario"}, {"value": "-0.021846858068456418", "module": "D", "scenario": "Standard scenario"}, {"name": "referenceToUnitGroupDataSet", "value": {"shortDescription": [{"value": "MJ", "lang": "en"}], "type": "unit group data set", "refObjectId": "93a60a57-a3c8-11da-a746-0800200c9a66", "version": "03.00.000", "uri": "../unitgroups/93a60a57-a3c8-11da-a746-0800200c9a66.xml"}}]}, "flowProperties": [], "typeOfFlow": "Other flow", "classification": {"classHierarchy": "Quantities", "name": "GaBiCategories"}}, {"dataSetInternalID": 15, "referenceToFlowDataSet": {"shortDescription": [{"value": "Use of renewable primary energy resources used as raw materials (PERM)", "lang": "en"}, {"value": "Erneuerbare Primärenergie zur stofflichen Nutzung (PERM)", "lang": "de"}, {"value": "Uso de energía primaria renovable utilizada como materia prima (PERM)", "lang": "es"}], "type": "flow data set", "refObjectId": "fb3ec0de-548d-4508-aea5-00b73bf6f702", "version": "38.00.000", "uri": "../flows/fb3ec0de-548d-4508-aea5-00b73bf6f702.xml"}, "exchange direction": "INPUT", "meanAmount": 0.0, "other": {"anies": [{"value": "18.453590099999893", "module": "A1", "scenario": "Standard scenario"}, {"value": "0.0", "module": "A2", "scenario": "Standard scenario"}, {"value": "0.46133975250000003", "module": "A3", "scenario": "Standard scenario"}, {"value": "18.914929852499892", "module": "A1-A3", "scenario": "Standard scenario"}, {"value": "0.0", "module": "C1", "scenario": "Standard scenario"}, {"value": "0.0", "module": "C2", "scenario": "Standard scenario"}, {"value": "0.0", "module": "C3", "scenario": "Standard scenario"}, {"value": "0.0", "module": "C4", "scenario": "Standard scenario"}, {"value": "0.0", "module": "D", "scenario": "Standard scenario"}, {"name": "referenceToUnitGroupDataSet", "value": {"shortDescription": [{"value": "MJ", "lang": "en"}], "type": "unit group data set", "refObjectId": "93a60a57-a3c8-11da-a746-0800200c9a66", "version": "03.00.000", "uri": "../unitgroups/93a60a57-a3c8-11da-a746-0800200c9a66.xml"}}]}, "flowProperties": [], "typeOfFlow": "Other flow", "classification": {"classHierarchy": "Quantities", "name": "GaBiCategories"}}, {"dataSetInternalID": 16, "referenceToFlowDataSet": {"shortDescription": [{"value": "Total use of renewable primary energy resources (PERT)", "lang": "en"}, {"value": "Total erneuerbare Primärenergie (PERT)", "lang": "de"}, {"value": "Uso total de la energía primaria renovable (energía primaria y recursos de energía primaria renovable utilizada como materia prima) (PERT)", "lang": "es"}], "type": "flow data set", "refObjectId": "53f97275-fa8a-4cdd-9024-65936002acd0", "version": "30.00.000", "uri": "../flows/53f97275-fa8a-4cdd-9024-65936002acd0.xml"}, "exchange direction": "INPUT", "meanAmount": 0.0, "other": {"anies": [{"value": "1.2096541048234", "module": "A1", "scenario": "Standard scenario"}, {"value": "0.014870255268576112", "module": "A2", "scenario": "Standard scenario"}, {"value": "0.4293815571829837", "module": "A3", "scenario": "Standard scenario"}, {"value": "1.65390591727496", "module": "A1-A3", "scenario": "Standard scenario"}, {"value": "2.440438130167E-4", "module": "C1", "scenario": "Standard scenario"}, {"value": "0.0038618095008182245", "module": "C2", "scenario": "Standard scenario"}, {"value": "0.172212884352", "module": "C3", "scenario": "Standard scenario"}, {"value": "9.859665024E-4", "module": "C4", "scenario": "Standard scenario"}, {"value": "-0.021846858068456418", "module": "D", "scenario": "Standard scenario"}, {"name": "referenceToUnitGroupDataSet", "value": {"shortDescription": [{"value": "MJ", "lang": "en"}], "type": "unit group data set", "refObjectId": "93a60a57-a3c8-11da-a746-0800200c9a66", "version": "03.00.000", "uri": "../unitgroups/93a60a57-a3c8-11da-a746-0800200c9a66.xml"}}]}, "flowProperties": [], "typeOfFlow": "Other flow", "classification": {"classHierarchy": "Größen / Umweltliche Größen / EPD EN 15804 / LCI Indikatoren", "name": "GaBiCategories"}}, {"dataSetInternalID": 17, "referenceToFlowDataSet": {"shortDescription": [{"value": "Use of renewable secondary fuels (RSF)", "lang": "en"}, {"value": "Erneuerbare Sekundärbrennstoffe (RSF)", "lang": "de"}, {"value": "Uso de combustibles secundarios renovables (RSF)", "lang": "es"}], "type": "flow data set", "refObjectId": "64333088-a55f-4aa2-9a31-c10b07816787", "version": "30.00.000", "uri": "../flows/64333088-a55f-4aa2-9a31-c10b07816787.xml"}, "exchange direction": "INPUT", "meanAmount": 0.0, "other": {"anies": [{"value": "0.0", "module": "A1", "scenario": "Standard scenario"}, {"value": "0.0", "module": "A2", "scenario": "Standard scenario"}, {"value": "0.0", "module": "A3", "scenario": "Standard scenario"}, {"value": "0.0", "module": "A1-A3", "scenario": "Standard scenario"}, {"value": "0.0", "module": "C1", "scenario": "Standard scenario"}, {"value": "0.0", "module": "C2", "scenario": "Standard scenario"}, {"value": "0.0", "module": "C3", "scenario": "Standard scenario"}, {"value": "0.0", "module": "C4", "scenario": "Standard scenario"}, {"value": "0.0", "module": "D", "scenario": "Standard scenario"}, {"name": "referenceToUnitGroupDataSet", "value": {"shortDescription": [{"value": "MJ", "lang": "en"}], "type": "unit group data set", "refObjectId": "93a60a57-a3c8-11da-a746-0800200c9a66", "version": "03.00.000", "uri": "../unitgroups/93a60a57-a3c8-11da-a746-0800200c9a66.xml"}}]}, "flowProperties": [], "typeOfFlow": "Other flow", "classification": {"classHierarchy": "Größen / Umweltliche Größen / EPD EN 15804 / LCI Indikatoren", "name": "GaBiCategories"}}, {"dataSetInternalID": 18, "referenceToFlowDataSet": {"shortDescription": [{"value": "Radioactive waste disposed (RWD)", "lang": "en"}, {"value": "Entsorgter radioaktiver Abfall (RWD)", "lang": "de"}, {"value": "Residuos radiactivos eliminados (RWD)", "lang": "es"}], "type": "flow data set", "refObjectId": "3449546e-52ad-4b39-b809-9fb77cea8ff6", "version": "30.00.000", "uri": "../flows/3449546e-52ad-4b39-b809-9fb77cea8ff6.xml"}, "exchange direction": "OUTPUT", "meanAmount": 0.0, "other": {"anies": [{"value": "3.3534650209990004E-5", "module": "A1", "scenario": "Standard scenario"}, {"value": "7.799718407746001E-6", "module": "A2", "scenario": "Standard scenario"}, {"value": "5.4391683826539995E-6", "module": "A3", "scenario": "Standard scenario"}, {"value": "4.6773537000390004E-5", "module": "A1-A3", "scenario": "Standard scenario"}, {"value": "3.132851896E-7", "module": "C1", "scenario": "Standard scenario"}, {"value": "2.0255890773540003E-6", "module": "C2", "scenario": "Standard scenario"}, {"value": "5.655126272E-6", "module": "C3", "scenario": "Standard scenario"}, {"value": "3.2259334400000004E-7", "module": "C4", "scenario": "Standard scenario"}, {"value": "-4.917941580780001E-6", "module": "D", "scenario": "Standard scenario"}, {"name": "referenceToUnitGroupDataSet", "value": {"shortDescription": [{"value": "kg", "lang": "en"}], "type": "unit group data set", "refObjectId": "ad38d542-3fe9-439d-9b95-2f5f7752acaf", "version": "30.00.000", "uri": "../unitgroups/ad38d542-3fe9-439d-9b95-2f5f7752acaf.xml"}}]}, "flowProperties": [], "typeOfFlow": "Other flow", "classification": {"classHierarchy": "Größen / Umweltliche Größen / EPD EN 15804 / LCI Indikatoren", "name": "GaBiCategories"}}, {"dataSetInternalID": 19, "referenceToFlowDataSet": {"shortDescription": [{"value": "Use of secondary material (SM)", "lang": "en"}, {"value": "Einsatz von Sekundärstoffen (SM)", "lang": "de"}, {"value": "Uso de materiales secundarios (SM)", "lang": "es"}], "type": "flow data set", "refObjectId": "c6a1f35f-2d09-4f54-8dfb-97e502e1ce92", "version": "30.00.000", "uri": "../flows/c6a1f35f-2d09-4f54-8dfb-97e502e1ce92.xml"}, "exchange direction": "INPUT", "meanAmount": 0.0, "other": {"anies": [{"value": "0.0", "module": "A1", "scenario": "Standard scenario"}, {"value": "0.0", "module": "A2", "scenario": "Standard scenario"}, {"value": "0.0", "module": "A3", "scenario": "Standard scenario"}, {"value": "0.0", "module": "A1-A3", "scenario": "Standard scenario"}, {"value": "0.0", "module": "C1", "scenario": "Standard scenario"}, {"value": "0.0", "module": "C2", "scenario": "Standard scenario"}, {"value": "0.0", "module": "C3", "scenario": "Standard scenario"}, {"value": "0.0", "module": "C4", "scenario": "Standard scenario"}, {"value": "0.0", "module": "D", "scenario": "Standard scenario"}, {"name": "referenceToUnitGroupDataSet", "value": {"shortDescription": [{"value": "kg", "lang": "en"}], "type": "unit group data set", "refObjectId": "ad38d542-3fe9-439d-9b95-2f5f7752acaf", "version": "30.00.000", "uri": "../unitgroups/ad38d542-3fe9-439d-9b95-2f5f7752acaf.xml"}}]}, "flowProperties": [], "typeOfFlow": "Other flow", "classification": {"classHierarchy": "Größen / Umweltliche Größen / EPD EN 15804 / LCI Indikatoren", "name": "GaBiCategories"}}]}, "LCIAResults": {"LCIAResult": [{"referenceToLCIAMethodDataSet": {"shortDescription": [{"value": "Abiotic depletion potential - non-fossil resources (ADPE)", "lang": "en"}, {"value": "Potenzial für die Verknappung abiotischer Ressourcen – nicht fossile Ressourcen (ADPE)", "lang": "de"}], "type": "LCIA method data set", "refObjectId": "b2ad6494-c78d-11e6-9d9d-cec0c932ce01", "version": "01.00.011", "uri": "../lciamethods/b2ad6494-c78d-11e6-9d9d-cec0c932ce01.xml"}, "meanAmount": 0.0, "other": {"anies": [{"value": "6.63062071041E-5", "module": "A1", "scenario": "Standard scenario"}, {"value": "1.995421192804E-6", "module": "A2", "scenario": "Standard scenario"}, {"value": "3.588405044444E-6", "module": "A3", "scenario": "Standard scenario"}, {"value": "7.1890033341348E-5", "module": "A1-A3", "scenario": "Standard scenario"}, {"value": "5.0275196E-9", "module": "C1", "scenario": "Standard scenario"}, {"value": "5.18211448346E-7", "module": "C2", "scenario": "Standard scenario"}, {"value": "2.7019898880000003E-6", "module": "C3", "scenario": "Standard scenario"}, {"value": "2.46816384E-8", "module": "C4", "scenario": "Standard scenario"}, {"value": "-1.62812954794E-7", "module": "D", "scenario": "Standard scenario"}, {"name": "referenceToUnitGroupDataSet", "value": {"shortDescription": [{"value": "kg Sb-eq.", "lang": "en"}], "type": "unit group data set", "refObjectId": "54ccd2d9-a32a-4fc2-923d-f2c8c93e89d4", "version": "30.00.000", "uri": "../unitgroups/54ccd2d9-a32a-4fc2-923d-f2c8c93e89d4.xml"}}]}}, {"referenceToLCIAMethodDataSet": {"shortDescription": [{"value": "Abiotic depletion potential - fossil resources (ADPF)", "lang": "en"}, {"value": "Potenzial für die Verknappung abiotischer Ressourcen – fossile Brennstoffe (ADPF)", "lang": "de"}], "type": "LCIA method data set", "refObjectId": "b2ad6110-c78d-11e6-9d9d-cec0c932ce01", "version": "01.00.011", "uri": "../lciamethods/b2ad6110-c78d-11e6-9d9d-cec0c932ce01.xml"}, "meanAmount": 0.0, "other": {"anies": [{"value": "104.2859455777459", "module": "A1", "scenario": "Standard scenario"}, {"value": "1.1877875438013374", "module": "A2", "scenario": "Standard scenario"}, {"value": "3.653148807604636", "module": "A3", "scenario": "Standard scenario"}, {"value": "109.12688192915188", "module": "A1-A3", "scenario": "Standard scenario"}, {"value": "0.0451182743782754", "module": "C1", "scenario": "Standard scenario"}, {"value": "0.30846876121210787", "module": "C2", "scenario": "Standard scenario"}, {"value": "1.5861130974207893", "module": "C3", "scenario": "Standard scenario"}, {"value": "0.0545472868864", "module": "C4", "scenario": "Standard scenario"}, {"value": "-10.287799405975656", "module": "D", "scenario": "Standard scenario"}, {"name": "referenceToUnitGroupDataSet", "value": {"shortDescription": [{"value": "MJ", "lang": "en"}], "type": "unit group data set", "refObjectId": "93a60a57-a3c8-11da-a746-0800200c9a66", "version": "03.00.000", "uri": "../unitgroups/93a60a57-a3c8-11da-a746-0800200c9a66.xml"}}]}}, {"referenceToLCIAMethodDataSet": {"shortDescription": [{"value": "Acidification potential, Accumulated Exceedance (AP)", "lang": "en"}, {"value": "Versauerungspotenzial, kumulierte Überschreitung (AP)", "lang": "de"}], "type": "LCIA method data set", "refObjectId": "b5c611c6-def3-11e6-bf01-fe55135034f3", "version": "01.03.010", "uri": "../lciamethods/b5c611c6-def3-11e6-bf01-fe55135034f3.xml"}, "meanAmount": 0.0, "other": {"anies": [{"value": "0.029639119774919002", "module": "A1", "scenario": "Standard scenario"}, {"value": "4.56760324680842E-4", "module": "A2", "scenario": "Standard scenario"}, {"value": "0.001169950109748302", "module": "A3", "scenario": "Standard scenario"}, {"value": "0.031265830209348144", "module": "A1-A3", "scenario": "Standard scenario"}, {"value": "3.42873756248E-5", "module": "C1", "scenario": "Standard scenario"}, {"value": "1.1862078556088801E-4", "module": "C2", "scenario": "Standard scenario"}, {"value": "9.820694016000001E-4", "module": "C3", "scenario": "Standard scenario"}, {"value": "2.026492416E-5", "module": "C4", "scenario": "Standard scenario"}, {"value": "-5.03444978490454E-4", "module": "D", "scenario": "Standard scenario"}, {"name": "referenceToUnitGroupDataSet", "value": {"shortDescription": [{"value": "mol H+-eq.", "lang": "en"}], "type": "unit group data set", "refObjectId": "42e089ac-92bf-4bf2-8ca1-5fc40d18f2ed", "version": "00.01.000", "uri": "../unitgroups/42e089ac-92bf-4bf2-8ca1-5fc40d18f2ed.xml"}}]}}, {"referenceToLCIAMethodDataSet": {"shortDescription": [{"value": "Eutrophication potential - freshwater (EP-freshwater)", "lang": "en"}, {"value": "Eutrophierungspotenzial - Süßwasser (EP-freshwater)", "lang": "de"}], "type": "LCIA method data set", "refObjectId": "b53ec18f-7377-4ad3-86eb-cc3f4f276b2b", "version": "01.00.011", "uri": "../lciamethods/b53ec18f-7377-4ad3-86eb-cc3f4f276b2b.xml"}, "meanAmount": 0.0, "other": {"anies": [{"value": "1.05997119397792E-4", "module": "A1", "scenario": "Standard scenario"}, {"value": "7.944553497480001E-7", "module": "A2", "scenario": "Standard scenario"}, {"value": "6.718542386028E-6", "module": "A3", "scenario": "Standard scenario"}, {"value": "1.13510117133568E-4", "module": "A1-A3", "scenario": "Standard scenario"}, {"value": "1.19341971E-8", "module": "C1", "scenario": "Standard scenario"}, {"value": "2.06320279114E-7", "module": "C2", "scenario": "Standard scenario"}, {"value": "6.633731584E-6", "module": "C3", "scenario": "Standard scenario"}, {"value": "4.20020864E-8", "module": "C4", "scenario": "Standard scenario"}, {"value": "-6.63081160834E-7", "module": "D", "scenario": "Standard scenario"}, {"name": "referenceToUnitGroupDataSet", "value": {"shortDescription": [{"value": "kg P-eq.", "lang": "en"}], "type": "unit group data set", "refObjectId": "0429039d-a61d-4590-ba67-aa4a20a810a1", "version": "30.00.000", "uri": "../unitgroups/0429039d-a61d-4590-ba67-aa4a20a810a1.xml"}}]}}, {"referenceToLCIAMethodDataSet": {"shortDescription": [{"value": "Eutrophication potential - marine (EP-marine)", "lang": "en"}, {"value": "Eutrophierungspotenzial - Salzwasser (EP-marine)", "lang": "de"}], "type": "LCIA method data set", "refObjectId": "b5c619fa-def3-11e6-bf01-fe55135034f3", "version": "02.00.011", "uri": "../lciamethods/b5c619fa-def3-11e6-bf01-fe55135034f3.xml"}, "meanAmount": 0.0, "other": {"anies": [{"value": "0.006513368105804201", "module": "A1", "scenario": "Standard scenario"}, {"value": "1.609513848797E-4", "module": "A2", "scenario": "Standard scenario"}, {"value": "2.2658071066152799E-4", "module": "A3", "scenario": "Standard scenario"}, {"value": "0.006900900201345428", "module": "A1-A3", "scenario": "Standard scenario"}, {"value": "1.51363791995E-5", "module": "C1", "scenario": "Standard scenario"}, {"value": "4.1799120194814006E-5", "module": "C2", "scenario": "Standard scenario"}, {"value": "2.68466944E-4", "module": "C3", "scenario": "Standard scenario"}, {"value": "1.643277504E-5", "module": "C4", "scenario": "Standard scenario"}, {"value": "-1.51258421345212E-4", "module": "D", "scenario": "Standard scenario"}, {"name": "referenceToUnitGroupDataSet", "value": {"shortDescription": [{"value": "kg N-eq.", "lang": "en"}], "type": "unit group data set", "refObjectId": "d05bb823-ecdf-4686-8c40-bf1d9257859f", "version": "00.00.003", "uri": "../unitgroups/d05bb823-ecdf-4686-8c40-bf1d9257859f.xml"}}]}}, {"referenceToLCIAMethodDataSet": {"shortDescription": [{"value": "Eutrophication potential - terrestrial (EP-terrestrial)", "lang": "en"}, {"value": "Eutrophierungspotenzial - Land (EP-terrestrial)", "lang": "de"}], "type": "LCIA method data set", "refObjectId": "b5c614d2-def3-11e6-bf01-fe55135034f3", "version": "01.02.010", "uri": "../lciamethods/b5c614d2-def3-11e6-bf01-fe55135034f3.xml"}, "meanAmount": 0.0, "other": {"anies": [{"value": "0.065120053723702", "module": "A1", "scenario": "Standard scenario"}, {"value": "0.0017745078156405061", "module": "A2", "scenario": "Standard scenario"}, {"value": "0.0023599453387229963", "module": "A3", "scenario": "Standard scenario"}, {"value": "0.0692545068780655", "module": "A1-A3", "scenario": "Standard scenario"}, {"value": "1.660810665023E-4", "module": "C1", "scenario": "Standard scenario"}, {"value": "4.6084018182243E-4", "module": "C2", "scenario": "Standard scenario"}, {"value": "0.0029903753472", "module": "C3", "scenario": "Standard scenario"}, {"value": "7.40449152E-5", "module": "C4", "scenario": "Standard scenario"}, {"value": "-0.001659398788563206", "module": "D", "scenario": "Standard scenario"}, {"name": "referenceToUnitGroupDataSet", "value": {"shortDescription": [{"value": "mol N-eq.", "lang": "en"}], "type": "unit group data set", "refObjectId": "71b4d617-0ec9-4d3f-b65e-e438940c2401", "version": "00.00.003", "uri": "../unitgroups/71b4d617-0ec9-4d3f-b65e-e438940c2401.xml"}}]}}, {"referenceToLCIAMethodDataSet": {"shortDescription": [{"value": "Potential Comparative Toxic Unit for ecosystems (ETP-fw)", "lang": "en"}, {"value": "Potenzielle Toxizitätsvergleichseinheit für Ökosysteme (ETP-fw)", "lang": "de"}], "type": "LCIA method data set", "refObjectId": "05316e7a-b254-4bea-9cf0-6bf33eb5c630", "version": "01.00.003", "uri": "../lciamethods/05316e7a-b254-4bea-9cf0-6bf33eb5c630.xml"}, "meanAmount": 0.0, "other": {"anies": [{"value": "21.080809476334014", "module": "A1", "scenario": "Standard scenario"}, {"value": "1.0591752457306303", "module": "A2", "scenario": "Standard scenario"}, {"value": "1.760480322440295", "module": "A3", "scenario": "Standard scenario"}, {"value": "23.90046504450494", "module": "A1-A3", "scenario": "Standard scenario"}, {"value": "0.0271982586007678", "module": "C1", "scenario": "Standard scenario"}, {"value": "0.27506811101203354", "module": "C2", "scenario": "Standard scenario"}, {"value": "28.95838609971189", "module": "C3", "scenario": "Standard scenario"}, {"value": "0.2048866104704", "module": "C4", "scenario": "Standard scenario"}, {"value": "-0.5961907331168489", "module": "D", "scenario": "Standard scenario"}, {"name": "referenceToUnitGroupDataSet", "value": {"shortDescription": [{"value": "CTUe", "lang": "en"}], "type": "unit group data set", "refObjectId": "aa959ded-f1eb-4efb-9c5c-2d60be36b3e6", "version": "00.00.003", "uri": "../unitgroups/aa959ded-f1eb-4efb-9c5c-2d60be36b3e6.xml"}}]}}, {"referenceToLCIAMethodDataSet": {"shortDescription": [{"value": "Global Warming Potential - biogenic (GWP-biogenic)", "lang": "en"}, {"value": "Globales Erwärmungspotenzial - biogen (GWP-biogenic)", "lang": "de"}], "type": "LCIA method data set", "refObjectId": "a7ea186c-9749-11ed-a8fc-0242ac120002", "version": "01.00.006", "uri": "../lciamethods/a7ea186c-9749-11ed-a8fc-0242ac120002.xml"}, "meanAmount": 0.0, "other": {"anies": [{"value": "0.013791494155625", "module": "A1", "scenario": "Standard scenario"}, {"value": "3.6357314607426005E-5", "module": "A2", "scenario": "Standard scenario"}, {"value": "6.740097846189605E-5", "module": "A3", "scenario": "Standard scenario"}, {"value": "0.013895252448694322", "module": "A1-A3", "scenario": "Standard scenario"}, {"value": "9.117507481E-7", "module": "C1", "scenario": "Standard scenario"}, {"value": "9.44200489096E-6", "module": "C2", "scenario": "Standard scenario"}, {"value": "4.3127915520000006E-4", "module": "C3", "scenario": "Standard scenario"}, {"value": "2.31660992E-5", "module": "C4", "scenario": "Standard scenario"}, {"value": "3.46933E-12", "module": "D", "scenario": "Standard scenario"}, {"name": "referenceToUnitGroupDataSet", "value": {"shortDescription": [{"value": "kg CO2-eq.", "lang": "en"}], "type": "unit group data set", "refObjectId": "1ebf3012-d0db-4de2-aefd-ef30cedb0be1", "version": "30.00.000", "uri": "../unitgroups/1ebf3012-d0db-4de2-aefd-ef30cedb0be1.xml"}}]}}, {"referenceToLCIAMethodDataSet": {"shortDescription": [{"value": "Global Warming Potential - fossil fuels (GWP-fossil)", "lang": "en"}, {"value": "Globales Erwärmungspotenzial - fossil (GWP-fossil)", "lang": "de"}], "type": "LCIA method data set", "refObjectId": "a7ea19c0-9749-11ed-a8fc-0242ac120002", "version": "01.00.009", "uri": "../lciamethods/a7ea19c0-9749-11ed-a8fc-0242ac120002.xml"}, "meanAmount": 0.0, "other": {"anies": [{"value": "7.8544686076501895", "module": "A1", "scenario": "Standard scenario"}, {"value": "0.07875535719724008", "module": "A2", "scenario": "Standard scenario"}, {"value": "0.3291779940406709", "module": "A3", "scenario": "Standard scenario"}, {"value": "8.2624019588881", "module": "A1-A3", "scenario": "Standard scenario"}, {"value": "0.0032781633982127", "module": "C1", "scenario": "Standard scenario"}, {"value": "0.02045278854811166", "module": "C2", "scenario": "Standard scenario"}, {"value": "2.3001277816832", "module": "C3", "scenario": "Standard scenario"}, {"value": "0.027750821785600004", "module": "C4", "scenario": "Standard scenario"}, {"value": "-0.6155023043917178", "module": "D", "scenario": "Standard scenario"}, {"name": "referenceToUnitGroupDataSet", "value": {"shortDescription": [{"value": "kg CO2-eq.", "lang": "en"}], "type": "unit group data set", "refObjectId": "1ebf3012-d0db-4de2-aefd-ef30cedb0be1", "version": "30.00.000", "uri": "../unitgroups/1ebf3012-d0db-4de2-aefd-ef30cedb0be1.xml"}}]}}, {"referenceToLCIAMethodDataSet": {"shortDescription": [{"value": "Global Warming Potential - land use and land use change (GWP-luluc)", "lang": "en"}, {"value": "Globales Erwärmungspotenzial - luluc (GWP-luluc)", "lang": "de"}], "type": "LCIA method data set", "refObjectId": "a7ea1ae2-9749-11ed-a8fc-0242ac120002", "version": "01.00.006", "uri": "../lciamethods/a7ea1ae2-9749-11ed-a8fc-0242ac120002.xml"}, "meanAmount": 0.0, "other": {"anies": [{"value": "6.265324090851001E-4", "module": "A1", "scenario": "Standard scenario"}, {"value": "2.88586180432E-5", "module": "A2", "scenario": "Standard scenario"}, {"value": "2.03442283288324E-4", "module": "A3", "scenario": "Standard scenario"}, {"value": "8.588333104166241E-4", "module": "A1-A3", "scenario": "Standard scenario"}, {"value": "2.583635492E-7", "module": "C1", "scenario": "Standard scenario"}, {"value": "7.494591271454001E-6", "module": "C2", "scenario": "Standard scenario"}, {"value": "1.7580254720000001E-4", "module": "C3", "scenario": "Standard scenario"}, {"value": "1.166965184E-6", "module": "C4", "scenario": "Standard scenario"}, {"value": "-1.7485915427682E-5", "module": "D", "scenario": "Standard scenario"}, {"name": "referenceToUnitGroupDataSet", "value": {"shortDescription": [{"value": "kg CO2-eq.", "lang": "en"}], "type": "unit group data set", "refObjectId": "1ebf3012-d0db-4de2-aefd-ef30cedb0be1", "version": "30.00.000", "uri": "../unitgroups/1ebf3012-d0db-4de2-aefd-ef30cedb0be1.xml"}}]}}, {"referenceToLCIAMethodDataSet": {"shortDescription": [{"value": "Global Warming Potential - total (GWP-total)", "lang": "en"}, {"value": "Globales Erwärmungspotenzial - total (GWP-total)", "lang": "de"}], "type": "LCIA method data set", "refObjectId": "a7ea142a-9749-11ed-a8fc-0242ac120002", "version": "04.00.017", "uri": "../lciamethods/a7ea142a-9749-11ed-a8fc-0242ac120002.xml"}, "meanAmount": 0.0, "other": {"anies": [{"value": "7.86888663964859", "module": "A1", "scenario": "Standard scenario"}, {"value": "0.0788205731298905", "module": "A2", "scenario": "Standard scenario"}, {"value": "0.32944883526564694", "module": "A3", "scenario": "Standard scenario"}, {"value": "8.277156048044127", "module": "A1-A3", "scenario": "Standard scenario"}, {"value": "0.0032793335125099", "module": "C1", "scenario": "Standard scenario"}, {"value": "0.020469725144273976", "module": "C2", "scenario": "Standard scenario"}, {"value": "2.30073486338559", "module": "C3", "scenario": "Standard scenario"}, {"value": "0.0277750704128", "module": "C4", "scenario": "Standard scenario"}, {"value": "-0.6155197903036759", "module": "D", "scenario": "Standard scenario"}, {"name": "referenceToUnitGroupDataSet", "value": {"shortDescription": [{"value": "kg CO2-eq.", "lang": "en"}], "type": "unit group data set", "refObjectId": "1ebf3012-d0db-4de2-aefd-ef30cedb0be1", "version": "30.00.000", "uri": "../unitgroups/1ebf3012-d0db-4de2-aefd-ef30cedb0be1.xml"}}]}}, {"referenceToLCIAMethodDataSet": {"shortDescription": [{"value": "Potential Comparative Toxic Unit for humans - cancer effects (HTP-c)", "lang": "en"}, {"value": "Potenzielle Toxizitätsvergleichseinheit für den Menschen - kanzerogene Wirkung (HTP-c)", "lang": "de"}], "type": "LCIA method data set", "refObjectId": "2299222a-bbd8-474f-9d4f-4dd1f18aea7c", "version": "01.00.004", "uri": "../lciamethods/2299222a-bbd8-474f-9d4f-4dd1f18aea7c.xml"}, "meanAmount": 0.0, "other": {"anies": [{"value": "1.1489377620000002E-9", "module": "A1", "scenario": "Standard scenario"}, {"value": "3.4353758E-11", "module": "A2", "scenario": "Standard scenario"}, {"value": "6.895657000000001E-11", "module": "A3", "scenario": "Standard scenario"}, {"value": "1.25224809E-9", "module": "A1-A3", "scenario": "Standard scenario"}, {"value": "9.505E-13", "module": "C1", "scenario": "Standard scenario"}, {"value": "8.921616E-12", "module": "C2", "scenario": "Standard scenario"}, {"value": "4.208868040000001E-10", "module": "C3", "scenario": "Standard scenario"}, {"value": "1.571826E-12", "module": "C4", "scenario": "Standard scenario"}, {"value": "-3.8767268E-11", "module": "D", "scenario": "Standard scenario"}, {"name": "referenceToUnitGroupDataSet", "value": {"shortDescription": [{"value": "CTUh", "lang": "en"}], "type": "unit group data set", "refObjectId": "d4c9523e-2d7e-49fd-8469-998f547d3a70", "version": "00.00.003", "uri": "../unitgroups/d4c9523e-2d7e-49fd-8469-998f547d3a70.xml"}}]}}, {"referenceToLCIAMethodDataSet": {"shortDescription": [{"value": "Potential Comparative Toxic Unit for humans - non-cancer effects (HTP-nc)", "lang": "en"}, {"value": "Potenzielle Toxizitätsvergleichseinheit für den Menschen - nicht kanzerogene Wirkung (HTP-nc)", "lang": "de"}], "type": "LCIA method data set", "refObjectId": "7cfdcfcf-b222-4b26-888a-a55f9fbf7ac8", "version": "01.00.003", "uri": "../lciamethods/7cfdcfcf-b222-4b26-888a-a55f9fbf7ac8.xml"}, "meanAmount": 0.0, "other": {"anies": [{"value": "2.4329359786E-8", "module": "A1", "scenario": "Standard scenario"}, {"value": "1.158578492E-9", "module": "A2", "scenario": "Standard scenario"}, {"value": "2.141804698E-9", "module": "A3", "scenario": "Standard scenario"}, {"value": "2.7629742975999997E-8", "module": "A1-A3", "scenario": "Standard scenario"}, {"value": "2.33565E-11", "module": "C1", "scenario": "Standard scenario"}, {"value": "3.0088322600000004E-10", "module": "C2", "scenario": "Standard scenario"}, {"value": "8.920030720000001E-9", "module": "C3", "scenario": "Standard scenario"}, {"value": "6.3436132E-11", "module": "C4", "scenario": "Standard scenario"}, {"value": "-5.48942618E-10", "module": "D", "scenario": "Standard scenario"}, {"name": "referenceToUnitGroupDataSet", "value": {"shortDescription": [{"value": "CTUh", "lang": "en"}], "type": "unit group data set", "refObjectId": "d4c9523e-2d7e-49fd-8469-998f547d3a70", "version": "00.00.003", "uri": "../unitgroups/d4c9523e-2d7e-49fd-8469-998f547d3a70.xml"}}]}}, {"referenceToLCIAMethodDataSet": {"shortDescription": [{"value": "Potential Human exposure efficiency relative to U235 (IRP)", "lang": "en"}, {"value": "Potenzielle Wirkung durch Exposition des Menschen mit U235 (IRP)", "lang": "de"}], "type": "LCIA method data set", "refObjectId": "b5c632be-def3-11e6-bf01-fe55135034f3", "version": "01.00.012", "uri": "../lciamethods/b5c632be-def3-11e6-bf01-fe55135034f3.xml"}, "meanAmount": 0.0, "other": {"anies": [{"value": "0.033165574107282006", "module": "A1", "scenario": "Standard scenario"}, {"value": "0.004976656196643156", "module": "A2", "scenario": "Standard scenario"}, {"value": "0.004422394652254888", "module": "A3", "scenario": "Standard scenario"}, {"value": "0.04256462495618005", "module": "A1-A3", "scenario": "Standard scenario"}, {"value": "1.933417855455E-4", "module": "C1", "scenario": "Standard scenario"}, {"value": "0.00129243902242312", "module": "C2", "scenario": "Standard scenario"}, {"value": "0.006737654272", "module": "C3", "scenario": "Standard scenario"}, {"value": "2.1347452160000002E-4", "module": "C4", "scenario": "Standard scenario"}, {"value": "-0.003309140392050482", "module": "D", "scenario": "Standard scenario"}, {"name": "referenceToUnitGroupDataSet", "value": {"shortDescription": [{"value": "kgBq U235-eq.", "lang": "en"}], "type": "unit group data set", "refObjectId": "456b05bf-1415-44a9-9993-02452f554c09", "version": "00.00.003", "uri": "../unitgroups/456b05bf-1415-44a9-9993-02452f554c09.xml"}}]}}, {"referenceToLCIAMethodDataSet": {"shortDescription": [{"value": "Depletion potential of the stratospheric ozone layer (ODP)", "lang": "en"}, {"value": "Abbaupotenzial der stratosphärischen Ozonschicht (ODP)", "lang": "de"}], "type": "LCIA method data set", "refObjectId": "b5c629d6-def3-11e6-bf01-fe55135034f3", "version": "02.00.013", "uri": "../lciamethods/b5c629d6-def3-11e6-bf01-fe55135034f3.xml"}, "meanAmount": 0.0, "other": {"anies": [{"value": "7.3715482812E-8", "module": "A1", "scenario": "Standard scenario"}, {"value": "1.7383198772E-8", "module": "A2", "scenario": "Standard scenario"}, {"value": "3.751189534E-9", "module": "A3", "scenario": "Standard scenario"}, {"value": "9.4849871118E-8", "module": "A1-A3", "scenario": "Standard scenario"}, {"value": "7.07951E-10", "module": "C1", "scenario": "Standard scenario"}, {"value": "4.51442166E-9", "module": "C2", "scenario": "Standard scenario"}, {"value": "6.936839424000001E-8", "module": "C3", "scenario": "Standard scenario"}, {"value": "7.10138368E-10", "module": "C4", "scenario": "Standard scenario"}, {"value": "-8.003143396E-8", "module": "D", "scenario": "Standard scenario"}, {"name": "referenceToUnitGroupDataSet", "value": {"shortDescription": [{"value": "kg CFC-11-eq.", "lang": "en"}], "type": "unit group data set", "refObjectId": "d9e957c9-7309-4474-bf3a-7777df6c4e5b", "version": "25.00.000", "uri": "../unitgroups/d9e957c9-7309-4474-bf3a-7777df6c4e5b.xml"}}]}}, {"referenceToLCIAMethodDataSet": {"shortDescription": [{"value": "Potential incidence of disease due to PM emissions (PM)", "lang": "en"}, {"value": "Potenzielles Auftreten von Krankheiten aufgrund von Feinstaubemissionen (PM)", "lang": "de"}], "type": "LCIA method data set", "refObjectId": "b5c602c6-def3-11e6-bf01-fe55135034f3", "version": "02.00.012", "uri": "../lciamethods/b5c602c6-def3-11e6-bf01-fe55135034f3.xml"}, "meanAmount": 0.0, "other": {"anies": [{"value": "2.72825435732E-7", "module": "A1", "scenario": "Standard scenario"}, {"value": "7.085114722E-9", "module": "A2", "scenario": "Standard scenario"}, {"value": "9.473523524000002E-9", "module": "A3", "scenario": "Standard scenario"}, {"value": "2.89384073978E-7", "module": "A1-A3", "scenario": "Standard scenario"}, {"value": "9.088843E-10", "module": "C1", "scenario": "Standard scenario"}, {"value": "1.8400062760000001E-9", "module": "C2", "scenario": "Standard scenario"}, {"value": "7.352530176E-9", "module": "C3", "scenario": "Standard scenario"}, {"value": "3.788848E-10", "module": "C4", "scenario": "Standard scenario"}, {"value": "-1.424705748E-9", "module": "D", "scenario": "Standard scenario"}, {"name": "referenceToUnitGroupDataSet", "value": {"shortDescription": [{"value": "Disease incidence", "lang": "en"}], "type": "unit group data set", "refObjectId": "3883559b-648f-4afc-8ba2-0bd24f3affa3", "version": "00.00.003", "uri": "../unitgroups/3883559b-648f-4afc-8ba2-0bd24f3affa3.xml"}}]}}, {"referenceToLCIAMethodDataSet": {"shortDescription": [{"value": "Photochemical Ozone Creation Potential (POCP)", "lang": "en"}, {"value": "Bildungspotenzial für troposphärisches Ozon (POCP)", "lang": "de"}], "type": "LCIA method data set", "refObjectId": "b5c610fe-def3-11e6-bf01-fe55135034f3", "version": "02.00.015", "uri": "../lciamethods/b5c610fe-def3-11e6-bf01-fe55135034f3.xml"}, "meanAmount": 0.0, "other": {"anies": [{"value": "0.022786809092058", "module": "A1", "scenario": "Standard scenario"}, {"value": "5.06634761696116E-4", "module": "A2", "scenario": "Standard scenario"}, {"value": "7.78102982088564E-4", "module": "A3", "scenario": "Standard scenario"}, {"value": "0.02407154683584268", "module": "A1-A3", "scenario": "Standard scenario"}, {"value": "4.56640738959E-5", "module": "C1", "scenario": "Standard scenario"}, {"value": "1.31573190965804E-4", "module": "C2", "scenario": "Standard scenario"}, {"value": "7.932765184E-4", "module": "C3", "scenario": "Standard scenario"}, {"value": "2.7279705600000002E-5", "module": "C4", "scenario": "Standard scenario"}, {"value": "-5.48632241962764E-4", "module": "D", "scenario": "Standard scenario"}, {"name": "referenceToUnitGroupDataSet", "value": {"shortDescription": [{"value": "kg NMVOC-eq.", "lang": "en"}], "type": "unit group data set", "refObjectId": "d27c25f8-fbc1-44c6-b47b-4adbae4199c6", "version": "00.00.003", "uri": "../unitgroups/d27c25f8-fbc1-44c6-b47b-4adbae4199c6.xml"}}]}}, {"referenceToLCIAMethodDataSet": {"shortDescription": [{"value": "Potential Soil quality index (SQP)", "lang": "en"}, {"value": "Potenzieller Bodenqualitätsindex (SQP)", "lang": "de"}], "type": "LCIA method data set", "refObjectId": "b2ad6890-c78d-11e6-9d9d-cec0c932ce01", "version": "01.00.011", "uri": "../lciamethods/b2ad6890-c78d-11e6-9d9d-cec0c932ce01.xml"}, "meanAmount": 0.0, "other": {"anies": [{"value": "3.1153328422558006", "module": "A1", "scenario": "Standard scenario"}, {"value": "1.030099624379878", "module": "A2", "scenario": "Standard scenario"}, {"value": "1.6388517061050105", "module": "A3", "scenario": "Standard scenario"}, {"value": "5.78428417274069", "module": "A1-A3", "scenario": "Standard scenario"}, {"value": "0.0057581609652561", "module": "C1", "scenario": "Standard scenario"}, {"value": "0.2675171639202371", "module": "C2", "scenario": "Standard scenario"}, {"value": "0.48664656529920003", "module": "C3", "scenario": "Standard scenario"}, {"value": "0.1284854648256", "module": "C4", "scenario": "Standard scenario"}, {"value": "-0.148003169612286", "module": "D", "scenario": "Standard scenario"}, {"name": "referenceToUnitGroupDataSet", "value": {"shortDescription": [{"value": "dimensionless", "lang": "en"}], "type": "unit group data set", "refObjectId": "f130951c-e67f-4f7f-8dd4-665de3974e18", "version": "00.00.004", "uri": "../unitgroups/f130951c-e67f-4f7f-8dd4-665de3974e18.xml"}}]}}, {"referenceToLCIAMethodDataSet": {"shortDescription": [{"value": "Water (user) deprivation potential (WDP)", "lang": "en"}, {"value": "Wasser-Entzugspotenzial (Benutzer) (WDP)", "lang": "de"}], "type": "LCIA method data set", "refObjectId": "b2ad66ce-c78d-11e6-9d9d-cec0c932ce01", "version": "03.00.015", "uri": "../lciamethods/b2ad66ce-c78d-11e6-9d9d-cec0c932ce01.xml"}, "meanAmount": 0.0, "other": {"anies": [{"value": "2.5736542954255888", "module": "A1", "scenario": "Standard scenario"}, {"value": "0.004249541299796077", "module": "A2", "scenario": "Standard scenario"}, {"value": "0.7022990163281714", "module": "A3", "scenario": "Standard scenario"}, {"value": "3.2802028530535563", "module": "A1-A3", "scenario": "Standard scenario"}, {"value": "6.04595515868E-5", "module": "C1", "scenario": "Standard scenario"}, {"value": "0.00110360707797342", "module": "C2", "scenario": "Standard scenario"}, {"value": "0.11416340288000001", "module": "C3", "scenario": "Standard scenario"}, {"value": "0.0023300332672000004", "module": "C4", "scenario": "Standard scenario"}, {"value": "-0.04476483442878555", "module": "D", "scenario": "Standard scenario"}, {"name": "referenceToUnitGroupDataSet", "value": {"shortDescription": [{"value": "m3 world eq. deprived", "lang": "en"}], "type": "unit group data set", "refObjectId": "6ae2df01-888e-46c8-b17d-49fa3869b476", "version": "00.00.003", "uri": "../unitgroups/6ae2df01-888e-46c8-b17d-49fa3869b476.xml"}}]}}]}, "otherAttributes": {"{http://www.indata.network/EPD/2019}epd-version": "1.2"}, "version": "1.1"}