{"processInformation": {"dataSetInformation": {"UUID": "ada97412-720d-4a00-85ec-99403cc5c947", "name": {"baseName": [{"value": "EverGuard TPO", "lang": "en"}, {"value": "EverGuard TPO", "lang": "de"}], "functionalUnitFlowProperties": [{"lang": "en"}]}, "classificationInformation": {"classification": [{"class": [{"value": "Kunststoffe", "level": 0, "classId": "6"}, {"value": "Dachbahnen", "level": 1, "classId": "6.3"}, {"value": "TPO-Dachbahnen (FPO)", "level": 2, "classId": "6.3.05"}], "name": "OEKOBAU.DAT"}, {"class": [{"value": "02 Building products", "level": 0}, {"value": "Membranes, including Liquid applied and kits", "level": 1}, {"value": "Plastic and elastomer roofing and sealing sheet systems", "level": 2}], "name": "IBUCategories"}]}, "generalComment": [{"value": "This EPD covers different EverGuard TPO roofing and sealing membranes which are closely described in the text below. For the LCA calculation in this declaration, an average of all 6 different EverGuard TPO products has been used. \nEverGuard TPO (1.1; 1.5; 2.0 mm) membranes are single-ply roofing products, designed to be used as an outer roof layer, either in new construction or re-covering applications. Fundamentally, all EverGuard TPO membranes are made of two layers of thermoplastic polyolefin (TPO) bonded to a layer of polyester scrim in the middle. This configuration meets all the inherent properties and performance which TPO is known for, including excellent seam strength, long-term weathering, reflectivity, and more.\n\nDifferent EverGuard TPO membranes share the same basic structure (as described above), with certain individual differences for a large number of different applications:\n\nEverGuard TPO FB (1.1; 1.5; 1.8; 2.0 mm)\nFleece backing\n\nEverGuard Extreme TPO (1.2; 1.5; 1.8; 2.0 mm)\nContains product modifications for an extended heat and UV resistance.\n\nEverGuard Extreme TPO FB (1.2; 1.5; 1.8; 2.0 mm) Contains a Fleece backing and product modifications for an extended heat and UV resistance.\n\nEverGuard Self Adhered TPO  (1.5; 2.0 mm)\nHot melt adhesive backing which increases the ease and time efficiency when fixing the membrane.\n\nEverGuard TPO T+ (1.2; 1.5; 1.8; 2.0 mm)\nContains product modifications with regard to extensive fire protection.", "lang": "en"}], "other": {"anies": [{"scenario": [{"description": [{"value": "Scenario 1", "lang": "en"}, {"value": "Szenario 1", "lang": "de"}], "name": "S1", "default": true}, {"description": [{"value": "Scenario 2", "lang": "en"}, {"value": "Szenario 2", "lang": "de"}], "name": "S2"}]}]}}, "quantitativeReference": {"referenceToReferenceFlow": [0]}, "time": {"referenceYear": 2025, "dataSetValidUntil": 2030, "other": {"anies": [{"name": "publicationDateOfEPD", "value": 1744848000000}]}}, "geography": {"locationOfOperationSupplyOrProduction": {"location": "RER"}}, "technology": {"technologyDescriptionAndIncludedProcesses": [{"value": "EverGuard TPO products are manufactured using an extrusion process. The polymers, performance-enhancing additives and other optional ingredients are fed into an extruder, which melts and homogenizes the added materials that are then extruded onto the top and bottom of a scrim to create laminated layers. The membrane is then cooled by passing through a series of rollers before being wound into rolls or cut to size and packaged for shipment. \nDeclared unit: \nThe declared unit is 1 m EverGuard TPO roofing membrane with a declared thickness of 1.5 mm; the factors for independent calculation of the values for different thicknesses are indicated in section 5. The sheets are laid loosely with ballast, fastened mechanically or through self-adherence. The seams are bonded through hot-air welding.", "lang": "en"}, {"lang": "de"}], "technologicalApplicability": [{"value": "EverGuard TPO products are designed as single-ply roofing solutions for use as an outer layer in both new construction and re-roofing applications.", "lang": "en"}, {"lang": "de"}]}}, "modellingAndValidation": {"LCIMethodAndAllocation": {"typeOfDataSet": "EPD", "referenceToLCAMethodDetails": [{"shortDescription": [{"value": "Plastic and elastomer roofing and sealing sheet systems.pdf", "lang": "en"}], "type": "source data set", "refObjectId": "00671302-a2a0-4b2e-897d-ee2efc35f3b9"}], "other": {"anies": [{"name": "subType", "value": "average dataset"}]}}, "dataSourcesTreatmentAndRepresentativeness": {"referenceToDataSource": [{"shortDescription": [{"value": "GaBi Database (all versions)", "lang": "en"}], "type": "source data set", "refObjectId": "28d74cc0-db8b-4d7e-bc44-5f6d56ce0c4a"}, {"shortDescription": [{"value": "Sphera MLC (fka GaBi) Databases Edition 2024", "lang": "en"}], "type": "source data set", "refObjectId": "7443b962-0446-4d69-8aa7-8055a6b1614a"}], "useAdviceForDataSet": [{"value": "Scope: \nThis Declaration applies for EverGuard TPO roofing and sealing membranes manufactured at 4 different GAF facilities in the USA. This declaration is valid for a range of EverGuard TPO products ( EverGuard TPO, EverGuard TPO FB, EverGuard Extreme TPO, EverGuard Extreme TPO FB, EverGuard SA TPO and EverGuard T+). \nThe LCA results are declared for an average EverGuard TPO membrane with a 1.5 mm thickness. \nSystem boundary: \nType of EPD: Cradle to gate with options, modules C1–C4, and module D (A1–A3 + C + D and additional modules A4 + A5)\n\nThe Life Cycle Assessment considers:\nA1-A5: Supply of raw materials and energy, raw material transport, product manufacturing, packaging material, transport to the building site and installation at the building site\nC1: Deconstruction and demolition\nC2/1: Transport to the recycling facility\nC2/2: Transport to the incineration facility\nC3/1: Waste processing (for recycling)\nC3/2: Incineration of waste\nD/1: Material credits from the recycling of the membrane\nD/2: Energy credits from the thermal treatment of the\npackaging material and product waste", "lang": "en"}], "other": {"anies": [{"name": "referenceToOriginalEPD", "value": {"shortDescription": {"value": "EverGuard TPO.pdf", "defaultValue": "EverGuard TPO.pdf", "lstrings": [{"lang": "en", "value": "EverGuard TPO.pdf"}]}, "type": "source data set", "uuid": {"uuid": "fbc9983f-27d0-4e22-bca5-053540030b41"}, "refObjectId": "fbc9983f-27d0-4e22-bca5-053540030b41", "resourceURLs": ["https://oekobaudat.de/OEKOBAU.DAT/resource/sources/fbc9983f-27d0-4e22-bca5-053540030b41/EverGuard_TPO_23828.pdf?version=00.02.000"]}}]}}, "validation": {"review": [{"referenceToNameOfReviewerAndInstitution": [{"shortDescription": [{"value": "Institut Bauen und Umwelt e. V.", "lang": "en"}], "type": "contact data set", "refObjectId": "d111dbec-b024-4be5-86c5-752d6eb2cf95", "uri": "../contacts/d111dbec-b024-4be5-86c5-752d6eb2cf95.xml"}], "type": "Accredited third party review"}]}, "complianceDeclarations": {"compliance": [{"referenceToComplianceSystem": {"shortDescription": [{"value": "DIN EN 15804+A2", "lang": "en"}], "type": "source data set", "refObjectId": "c0016b33-8cf7-415c-ac6e-deba0d21440d", "uri": "../sources/c0016b33-8cf7-415c-ac6e-deba0d21440d.xml"}}, {"referenceToComplianceSystem": {"shortDescription": [{"value": "ISO 14025", "lang": "en"}], "type": "source data set", "refObjectId": "4f2eb655-6e44-4874-a95a-e28f5442cd4d", "uri": "../sources/4f2eb655-6e44-4874-a95a-e28f5442cd4d.xml"}}]}}, "administrativeInformation": {"commissionerAndGoal": {"referenceToCommissioner": [{"shortDescription": [{"value": "BMI Group Holdings UK Ltd", "lang": "en"}], "type": "contact data set", "refObjectId": "86642c3f-c4f6-42f9-bca9-609227beae5b", "uri": "../contacts/86642c3f-c4f6-42f9-bca9-609227beae5b.xml"}]}, "dataGenerator": {"referenceToPersonOrEntityGeneratingTheDataSet": [{"shortDescription": [{"value": "BMI Deutschland", "lang": "en"}], "type": "contact data set", "refObjectId": "320bf93e-9d3f-4ce3-9648-2efe638e005f", "uri": "../contacts/320bf93e-9d3f-4ce3-9648-2efe638e005f.xml"}]}, "dataEntryBy": {"timeStamp": 1744848000000, "referenceToDataSetFormat": [{"shortDescription": [{"value": "ILCD Format", "lang": "en"}], "type": "source data set", "refObjectId": "a97a0155-0234-4b87-b4ce-a45da52f2a40", "uri": "../sources/a97a0155-0234-4b87-b4ce-a45da52f2a40.xml"}, {"shortDescription": [{"value": "EPD-Datenformaterweiterungen v1.2", "lang": "de"}, {"value": "EPD Data Format Extensions v1.2", "lang": "en"}], "type": "source data set", "refObjectId": "a29449fd-aa2f-4de8-b5d7-4b06b43c6fde", "uri": "../sources/a29449fd-aa2f-4de8-b5d7-4b06b43c6fde.xml"}]}, "publicationAndOwnership": {"dataSetVersion": "00.03.000", "referenceToRegistrationAuthority": {"shortDescription": [{"value": "Institut Bauen und Umwelt e. V.", "lang": "en"}], "type": "contact data set", "refObjectId": "d111dbec-b024-4be5-86c5-752d6eb2cf95", "uri": "../contacts/d111dbec-b024-4be5-86c5-752d6eb2cf95.xml"}, "registrationNumber": "EPD-WOL-20250076-IBC1-EN", "referenceToOwnershipOfDataSet": {"shortDescription": [{"value": "BMI Group Holdings UK Ltd", "lang": "en"}], "type": "contact data set", "refObjectId": "86642c3f-c4f6-42f9-bca9-609227beae5b", "uri": "../contacts/86642c3f-c4f6-42f9-bca9-609227beae5b.xml"}, "copyright": true, "licenseType": "Free of charge for all users and uses", "accessRestrictions": [{"value": "None", "lang": "en"}], "other": {"anies": [{"name": "referenceToPublisher", "value": {"shortDescription": [{"value": "Institut Bauen und Umwelt e. V.", "lang": "en"}], "type": "contact data set", "refObjectId": "d111dbec-b024-4be5-86c5-752d6eb2cf95", "uri": "../contacts/d111dbec-b024-4be5-86c5-752d6eb2cf95.xml"}}]}}}, "exchanges": {"exchange": [{"dataSetInternalID": 0, "referenceToFlowDataSet": {"shortDescription": [{"value": "EverGuard TPO (EverGuard TPO)", "lang": "en"}], "type": "flow data set", "refObjectId": "f786fc80-6ed5-bfe2-d727-1ff95fa1081e", "uri": "../flows/f786fc80-6ed5-bfe2-d727-1ff95fa1081e.xml"}, "meanAmount": 1.0, "referencesToDataSource": {}, "referenceFlow": true, "resolvedFlowVersion": "00.03.000", "resultingflowAmount": 1.0, "flowProperties": [{"name": [{"lang": "de", "value": "Fläche"}, {"lang": "en", "value": "Area"}], "uuid": "93a60a56-a3c8-19da-a746-0800200c9a66", "referenceFlowProperty": true, "meanValue": 1.0, "referenceUnit": "qm", "unitGroupUUID": "c20a03d7-bd90-4569-bc94-66cfd364dfc8"}], "materialProperties": [{"name": "conversion factor to 1 kg", "value": "0.625", "unit": "-", "unitDescription": "Without unit"}, {"name": "layer thickness", "value": "0.0015", "unit": "m", "unitDescription": "meters"}, {"name": "grammage", "value": "1.6", "unit": "kg/m^2", "unitDescription": "kilograms per square meter"}], "typeOfFlow": "Product flow", "classification": {"classHierarchy": "Kunststoffe / Dachbahnen / TPO-Dachbahnen (FPO)", "name": "OEKOBAU.DAT"}}, {"dataSetInternalID": 1, "referenceToFlowDataSet": {"shortDescription": [{"value": "Renewable primary energy as energy carrier (PERE)", "lang": "en"}, {"value": "Erneuerbare Primärenergie als Energieträger (PERE)", "lang": "de"}], "type": "flow data set", "refObjectId": "20f32be5-0398-4288-9b6d-accddd195317", "uri": "../flows/20f32be5-0398-4288-9b6d-accddd195317.xml"}, "exchange direction": "INPUT", "other": {"anies": [{"name": "referenceToUnitGroupDataSet", "value": {"shortDescription": [{"value": "MJ", "lang": "en"}], "type": "unit group data set", "refObjectId": "93a60a57-a3c8-11da-a746-0800200c9a66", "uri": "../unitgroups/93a60a57-a3c8-11da-a746-0800200c9a66.xml"}}, {"value": "4.9092", "module": "A1-A3"}, {"value": "0.18", "module": "A4"}, {"value": "0.973", "module": "A5"}, {"value": "0", "module": "C1"}, {"value": "0.018", "module": "C2", "scenario": "S1"}, {"value": "0.018", "module": "C2", "scenario": "S2"}, {"value": "3.99", "module": "C3", "scenario": "S1"}, {"value": "1.29", "module": "C3", "scenario": "S2"}, {"value": "-4.17", "module": "D", "scenario": "S1"}, {"value": "-6.47", "module": "D", "scenario": "S2"}]}, "resolvedFlowVersion": "38.00.000", "flowProperties": [], "typeOfFlow": "Other flow", "classification": {"classHierarchy": "Quantities", "name": "GaBiCategories"}}, {"dataSetInternalID": 2, "referenceToFlowDataSet": {"shortDescription": [{"value": "Renewable primary energy resources as material utilization (PERM)", "lang": "en"}, {"value": "Erneuerbare Primärenergie zur stofflichen Nutzung (PERM)", "lang": "de"}], "type": "flow data set", "refObjectId": "fb3ec0de-548d-4508-aea5-00b73bf6f702", "uri": "../flows/fb3ec0de-548d-4508-aea5-00b73bf6f702.xml"}, "exchange direction": "INPUT", "other": {"anies": [{"name": "referenceToUnitGroupDataSet", "value": {"shortDescription": [{"value": "MJ", "lang": "en"}], "type": "unit group data set", "refObjectId": "93a60a57-a3c8-11da-a746-0800200c9a66", "uri": "../unitgroups/93a60a57-a3c8-11da-a746-0800200c9a66.xml"}}, {"value": "0.284", "module": "A1-A3"}, {"value": "0", "module": "A4"}, {"value": "-0.284", "module": "A5"}, {"value": "0", "module": "C1"}, {"value": "0", "module": "C2", "scenario": "S1"}, {"value": "0", "module": "C2", "scenario": "S2"}, {"value": "0", "module": "C3", "scenario": "S1"}, {"value": "0", "module": "C3", "scenario": "S2"}, {"value": "0", "module": "D", "scenario": "S1"}, {"value": "0", "module": "D", "scenario": "S2"}]}, "resolvedFlowVersion": "38.00.000", "flowProperties": [], "typeOfFlow": "Other flow", "classification": {"classHierarchy": "Quantities", "name": "GaBiCategories"}}, {"dataSetInternalID": 3, "referenceToFlowDataSet": {"shortDescription": [{"value": "Total use of renewable primary energy resources (PERT)", "lang": "en"}, {"value": "Total erneuerbare Primärenergie (PERT)", "lang": "de"}], "type": "flow data set", "refObjectId": "53f97275-fa8a-4cdd-9024-65936002acd0", "uri": "../flows/53f97275-fa8a-4cdd-9024-65936002acd0.xml"}, "exchange direction": "INPUT", "other": {"anies": [{"name": "referenceToUnitGroupDataSet", "value": {"shortDescription": [{"value": "MJ", "lang": "en"}], "type": "unit group data set", "refObjectId": "93a60a57-a3c8-11da-a746-0800200c9a66", "uri": "../unitgroups/93a60a57-a3c8-11da-a746-0800200c9a66.xml"}}, {"value": "5.1912", "module": "A1-A3"}, {"value": "0.18", "module": "A4"}, {"value": "0.689", "module": "A5"}, {"value": "0", "module": "C1"}, {"value": "0.018", "module": "C2", "scenario": "S1"}, {"value": "0.018", "module": "C2", "scenario": "S2"}, {"value": "3.99", "module": "C3", "scenario": "S1"}, {"value": "1.29", "module": "C3", "scenario": "S2"}, {"value": "-4.17", "module": "D", "scenario": "S1"}, {"value": "-6.47", "module": "D", "scenario": "S2"}]}, "resolvedFlowVersion": "38.00.000", "flowProperties": [], "typeOfFlow": "Other flow", "classification": {"classHierarchy": "Quantities / Environmental quantities / EPD EN 15804 / LCI indicators", "name": "GaBiCategories"}}, {"dataSetInternalID": 4, "referenceToFlowDataSet": {"shortDescription": [{"value": "Non renewable primary energy as energy carrier (PENRE)", "lang": "en"}, {"value": "Nicht-erneuerbare Primärenergie als Energieträger (PENRE)", "lang": "de"}], "type": "flow data set", "refObjectId": "ac857178-2b45-46ec-892a-a9a4332f0372", "uri": "../flows/ac857178-2b45-46ec-892a-a9a4332f0372.xml"}, "exchange direction": "INPUT", "other": {"anies": [{"name": "referenceToUnitGroupDataSet", "value": {"shortDescription": [{"value": "MJ", "lang": "en"}], "type": "unit group data set", "refObjectId": "93a60a57-a3c8-11da-a746-0800200c9a66", "uri": "../unitgroups/93a60a57-a3c8-11da-a746-0800200c9a66.xml"}}, {"value": "46.279", "module": "A1-A3"}, {"value": "2.92", "module": "A4"}, {"value": "16.6", "module": "A5"}, {"value": "0", "module": "C1"}, {"value": "0.163", "module": "C2", "scenario": "S1"}, {"value": "0.163", "module": "C2", "scenario": "S2"}, {"value": "66.9", "module": "C3", "scenario": "S1"}, {"value": "65.6", "module": "C3", "scenario": "S2"}, {"value": "-106", "module": "D", "scenario": "S1"}, {"value": "-19.7", "module": "D", "scenario": "S2"}]}, "resolvedFlowVersion": "38.00.000", "flowProperties": [], "typeOfFlow": "Other flow", "classification": {"classHierarchy": "Quantities", "name": "GaBiCategories"}}, {"dataSetInternalID": 5, "referenceToFlowDataSet": {"shortDescription": [{"value": "Non renewable primary energy as material utilization (PENRM)", "lang": "en"}, {"value": "Nicht-erneuerbare Primärenergie zur stofflichen Nutzung (PENRM)", "lang": "de"}], "type": "flow data set", "refObjectId": "1421caa0-679d-4bf4-b282-0eb850ccae27", "uri": "../flows/1421caa0-679d-4bf4-b282-0eb850ccae27.xml"}, "exchange direction": "INPUT", "other": {"anies": [{"name": "referenceToUnitGroupDataSet", "value": {"shortDescription": [{"value": "MJ", "lang": "en"}], "type": "unit group data set", "refObjectId": "93a60a57-a3c8-11da-a746-0800200c9a66", "uri": "../unitgroups/93a60a57-a3c8-11da-a746-0800200c9a66.xml"}}, {"value": "69.34", "module": "A1-A3"}, {"value": "0", "module": "A4"}, {"value": "-8.84", "module": "A5"}, {"value": "0", "module": "C1"}, {"value": "0", "module": "C2", "scenario": "S1"}, {"value": "0", "module": "C2", "scenario": "S2"}, {"value": "-60.5", "module": "C3", "scenario": "S1"}, {"value": "-60.5", "module": "C3", "scenario": "S2"}, {"value": "0", "module": "D", "scenario": "S1"}, {"value": "0", "module": "D", "scenario": "S2"}]}, "resolvedFlowVersion": "38.00.000", "flowProperties": [], "typeOfFlow": "Other flow", "classification": {"classHierarchy": "Quantities", "name": "GaBiCategories"}}, {"dataSetInternalID": 6, "referenceToFlowDataSet": {"shortDescription": [{"value": "Total use of non renewable primary energy resources (PENRT)", "lang": "en"}, {"value": "Total nicht erneuerbare Primärenergie (PENRT)", "lang": "de"}], "type": "flow data set", "refObjectId": "06159210-646b-4c8d-8583-da9b3b95a6c1", "uri": "../flows/06159210-646b-4c8d-8583-da9b3b95a6c1.xml"}, "exchange direction": "INPUT", "other": {"anies": [{"name": "referenceToUnitGroupDataSet", "value": {"shortDescription": [{"value": "MJ", "lang": "en"}], "type": "unit group data set", "refObjectId": "93a60a57-a3c8-11da-a746-0800200c9a66", "uri": "../unitgroups/93a60a57-a3c8-11da-a746-0800200c9a66.xml"}}, {"value": "115.409", "module": "A1-A3"}, {"value": "2.92", "module": "A4"}, {"value": "7.79", "module": "A5"}, {"value": "0", "module": "C1"}, {"value": "0.163", "module": "C2", "scenario": "S1"}, {"value": "0.163", "module": "C2", "scenario": "S2"}, {"value": "6.34", "module": "C3", "scenario": "S1"}, {"value": "5.04", "module": "C3", "scenario": "S2"}, {"value": "-106", "module": "D", "scenario": "S1"}, {"value": "-19.7", "module": "D", "scenario": "S2"}]}, "resolvedFlowVersion": "38.00.000", "flowProperties": [], "typeOfFlow": "Other flow", "classification": {"classHierarchy": "Quantities / Environmental quantities / EPD EN 15804 / LCI indicators", "name": "GaBiCategories"}}, {"dataSetInternalID": 7, "referenceToFlowDataSet": {"shortDescription": [{"value": "Use of secondary material (SM)", "lang": "en"}, {"value": "Einsatz von Sekundärstoffen (SM)", "lang": "de"}], "type": "flow data set", "refObjectId": "c6a1f35f-2d09-4f54-8dfb-97e502e1ce92", "uri": "../flows/c6a1f35f-2d09-4f54-8dfb-97e502e1ce92.xml"}, "exchange direction": "INPUT", "other": {"anies": [{"name": "referenceToUnitGroupDataSet", "value": {"shortDescription": [{"value": "kg", "lang": "en"}], "type": "unit group data set", "refObjectId": "ad38d542-3fe9-439d-9b95-2f5f7752acaf", "uri": "../unitgroups/ad38d542-3fe9-439d-9b95-2f5f7752acaf.xml"}}, {"value": "0", "module": "A1-A3"}, {"value": "0", "module": "A4"}, {"value": "0", "module": "A5"}, {"value": "0", "module": "C1"}, {"value": "0", "module": "C2", "scenario": "S1"}, {"value": "0", "module": "C2", "scenario": "S2"}, {"value": "0", "module": "C3", "scenario": "S1"}, {"value": "0", "module": "C3", "scenario": "S2"}, {"value": "-1.47", "module": "D", "scenario": "S1"}, {"value": "0", "module": "D", "scenario": "S2"}]}, "resolvedFlowVersion": "38.00.000", "flowProperties": [], "typeOfFlow": "Other flow", "classification": {"classHierarchy": "Quantities / Environmental quantities / EPD EN 15804 / LCI indicators", "name": "GaBiCategories"}}, {"dataSetInternalID": 8, "referenceToFlowDataSet": {"shortDescription": [{"value": "Use of renewable secondary fuels (RSF)", "lang": "en"}, {"value": "Erneuerbare Sekundärbrennstoffe (RSF)", "lang": "de"}], "type": "flow data set", "refObjectId": "64333088-a55f-4aa2-9a31-c10b07816787", "uri": "../flows/64333088-a55f-4aa2-9a31-c10b07816787.xml"}, "exchange direction": "INPUT", "other": {"anies": [{"name": "referenceToUnitGroupDataSet", "value": {"shortDescription": [{"value": "MJ", "lang": "en"}], "type": "unit group data set", "refObjectId": "93a60a57-a3c8-11da-a746-0800200c9a66", "uri": "../unitgroups/93a60a57-a3c8-11da-a746-0800200c9a66.xml"}}, {"value": "0", "module": "A1-A3"}, {"value": "0", "module": "A4"}, {"value": "0", "module": "A5"}, {"value": "0", "module": "C1"}, {"value": "0", "module": "C2", "scenario": "S1"}, {"value": "0", "module": "C2", "scenario": "S2"}, {"value": "0", "module": "C3", "scenario": "S1"}, {"value": "0", "module": "C3", "scenario": "S2"}, {"value": "0", "module": "D", "scenario": "S1"}, {"value": "0", "module": "D", "scenario": "S2"}]}, "resolvedFlowVersion": "38.00.000", "flowProperties": [], "typeOfFlow": "Other flow", "classification": {"classHierarchy": "Quantities / Environmental quantities / EPD EN 15804 / LCI indicators", "name": "GaBiCategories"}}, {"dataSetInternalID": 9, "referenceToFlowDataSet": {"shortDescription": [{"value": "Use of non renewable secondary fuels (NRSF)", "lang": "en"}, {"value": "Nicht erneuerbare Sekundärbrennstoffe (NRSF)", "lang": "de"}], "type": "flow data set", "refObjectId": "89def144-d39a-4287-b86f-efde453ddcb2", "uri": "../flows/89def144-d39a-4287-b86f-efde453ddcb2.xml"}, "exchange direction": "INPUT", "other": {"anies": [{"name": "referenceToUnitGroupDataSet", "value": {"shortDescription": [{"value": "MJ", "lang": "en"}], "type": "unit group data set", "refObjectId": "93a60a57-a3c8-11da-a746-0800200c9a66", "uri": "../unitgroups/93a60a57-a3c8-11da-a746-0800200c9a66.xml"}}, {"value": "0", "module": "A1-A3"}, {"value": "0", "module": "A4"}, {"value": "0", "module": "A5"}, {"value": "0", "module": "C1"}, {"value": "0", "module": "C2", "scenario": "S1"}, {"value": "0", "module": "C2", "scenario": "S2"}, {"value": "0", "module": "C3", "scenario": "S1"}, {"value": "0", "module": "C3", "scenario": "S2"}, {"value": "0", "module": "D", "scenario": "S1"}, {"value": "0", "module": "D", "scenario": "S2"}]}, "resolvedFlowVersion": "38.00.000", "flowProperties": [], "typeOfFlow": "Other flow", "classification": {"classHierarchy": "Quantities / Environmental quantities / EPD EN 15804 / LCI indicators", "name": "GaBiCategories"}}, {"dataSetInternalID": 10, "referenceToFlowDataSet": {"shortDescription": [{"value": "Use of net fresh water (FW)", "lang": "en"}, {"value": "Einsatz von Süßwasserressourcen (FW)", "lang": "de"}], "type": "flow data set", "refObjectId": "3cf952c8-f3a4-461d-8c96-96456ca62246", "uri": "../flows/3cf952c8-f3a4-461d-8c96-96456ca62246.xml"}, "exchange direction": "INPUT", "other": {"anies": [{"name": "referenceToUnitGroupDataSet", "value": {"shortDescription": [{"value": "m^3", "lang": "en"}], "type": "unit group data set", "refObjectId": "cd950537-0a98-4044-9ba7-9f9a68d0a504", "uri": "../unitgroups/cd950537-0a98-4044-9ba7-9f9a68d0a504.xml"}}, {"value": "0.0615305", "module": "A1-A3"}, {"value": "0.000175", "module": "A4"}, {"value": "0.00516", "module": "A5"}, {"value": "0", "module": "C1"}, {"value": "1.68E-05", "module": "C2", "scenario": "S1"}, {"value": "1.68E-05", "module": "C2", "scenario": "S2"}, {"value": "0.00345", "module": "C3", "scenario": "S1"}, {"value": "0.00802", "module": "C3", "scenario": "S2"}, {"value": "-0.0116", "module": "D", "scenario": "S1"}, {"value": "-0.00497", "module": "D", "scenario": "S2"}]}, "resolvedFlowVersion": "38.00.000", "flowProperties": [], "typeOfFlow": "Other flow", "classification": {"classHierarchy": "Quantities / Environmental quantities / EPD EN 15804 / LCI indicators", "name": "GaBiCategories"}}, {"dataSetInternalID": 11, "referenceToFlowDataSet": {"shortDescription": [{"value": "Hazardous waste disposed (HWD)", "lang": "en"}, {"value": "Gefährlicher Abfall zur Deponie (HWD)", "lang": "de"}], "type": "flow data set", "refObjectId": "430f9e0f-59b2-46a0-8e0d-55e0e84948fc", "uri": "../flows/430f9e0f-59b2-46a0-8e0d-55e0e84948fc.xml"}, "exchange direction": "OUTPUT", "other": {"anies": [{"name": "referenceToUnitGroupDataSet", "value": {"shortDescription": [{"value": "kg", "lang": "en"}], "type": "unit group data set", "refObjectId": "ad38d542-3fe9-439d-9b95-2f5f7752acaf", "uri": "../unitgroups/ad38d542-3fe9-439d-9b95-2f5f7752acaf.xml"}}, {"value": "6.9817146E-06", "module": "A1-A3"}, {"value": "2.66E-10", "module": "A4"}, {"value": "4.31E-07", "module": "A5"}, {"value": "0", "module": "C1"}, {"value": "7.92E-12", "module": "C2", "scenario": "S1"}, {"value": "7.92E-12", "module": "C2", "scenario": "S2"}, {"value": "2E-07", "module": "C3", "scenario": "S1"}, {"value": "2.82E-09", "module": "C3", "scenario": "S2"}, {"value": "-9.95E-09", "module": "D", "scenario": "S1"}, {"value": "-1.31E-08", "module": "D", "scenario": "S2"}]}, "resolvedFlowVersion": "38.00.000", "flowProperties": [], "typeOfFlow": "Other flow", "classification": {"classHierarchy": "Quantities / Environmental quantities / EPD EN 15804 / LCI indicators", "name": "GaBiCategories"}}, {"dataSetInternalID": 12, "referenceToFlowDataSet": {"shortDescription": [{"value": "Non hazardous waste disposed (NHWD)", "lang": "en"}, {"value": "Entsorgter nicht gefährlicher Abfall (NHWD)", "lang": "de"}], "type": "flow data set", "refObjectId": "b29ef66b-e286-4afa-949f-62f1a7b4d7fa", "uri": "../flows/b29ef66b-e286-4afa-949f-62f1a7b4d7fa.xml"}, "exchange direction": "OUTPUT", "other": {"anies": [{"name": "referenceToUnitGroupDataSet", "value": {"shortDescription": [{"value": "kg", "lang": "en"}], "type": "unit group data set", "refObjectId": "ad38d542-3fe9-439d-9b95-2f5f7752acaf", "uri": "../unitgroups/ad38d542-3fe9-439d-9b95-2f5f7752acaf.xml"}}, {"value": "0.8097678", "module": "A1-A3"}, {"value": "0.000336", "module": "A4"}, {"value": "0.114", "module": "A5"}, {"value": "0", "module": "C1"}, {"value": "2.75E-05", "module": "C2", "scenario": "S1"}, {"value": "2.75E-05", "module": "C2", "scenario": "S2"}, {"value": "0.175", "module": "C3", "scenario": "S1"}, {"value": "1.37", "module": "C3", "scenario": "S2"}, {"value": "-0.0262", "module": "D", "scenario": "S1"}, {"value": "-0.0102", "module": "D", "scenario": "S2"}]}, "resolvedFlowVersion": "38.00.000", "flowProperties": [], "typeOfFlow": "Other flow", "classification": {"classHierarchy": "Quantities / Environmental quantities / EPD EN 15804 / LCI indicators", "name": "GaBiCategories"}}, {"dataSetInternalID": 13, "referenceToFlowDataSet": {"shortDescription": [{"value": "Radioactive waste disposed (RWD)", "lang": "en"}, {"value": "Entsorgter radioaktiver Abfall (RWD)", "lang": "de"}], "type": "flow data set", "refObjectId": "3449546e-52ad-4b39-b809-9fb77cea8ff6", "uri": "../flows/3449546e-52ad-4b39-b809-9fb77cea8ff6.xml"}, "exchange direction": "OUTPUT", "other": {"anies": [{"name": "referenceToUnitGroupDataSet", "value": {"shortDescription": [{"value": "kg", "lang": "en"}], "type": "unit group data set", "refObjectId": "ad38d542-3fe9-439d-9b95-2f5f7752acaf", "uri": "../unitgroups/ad38d542-3fe9-439d-9b95-2f5f7752acaf.xml"}}, {"value": "0.00248145", "module": "A1-A3"}, {"value": "6.32E-06", "module": "A4"}, {"value": "0.000216", "module": "A5"}, {"value": "0", "module": "C1"}, {"value": "2.59E-07", "module": "C2", "scenario": "S1"}, {"value": "2.59E-07", "module": "C2", "scenario": "S2"}, {"value": "0.000877", "module": "C3", "scenario": "S1"}, {"value": "0.000131", "module": "C3", "scenario": "S2"}, {"value": "-0.000708", "module": "D", "scenario": "S1"}, {"value": "-0.00143", "module": "D", "scenario": "S2"}]}, "resolvedFlowVersion": "38.00.000", "flowProperties": [], "typeOfFlow": "Other flow", "classification": {"classHierarchy": "Quantities / Environmental quantities / EPD EN 15804 / LCI indicators", "name": "GaBiCategories"}}, {"dataSetInternalID": 14, "referenceToFlowDataSet": {"shortDescription": [{"value": "Components for re-use (CRU)", "lang": "en"}, {"value": "Komponenten für die Wiederverwendung (CRU)", "lang": "de"}], "type": "flow data set", "refObjectId": "a2b32f97-3fc7-4af2-b209-525bc6426f33", "uri": "../flows/a2b32f97-3fc7-4af2-b209-525bc6426f33.xml"}, "exchange direction": "OUTPUT", "other": {"anies": [{"name": "referenceToUnitGroupDataSet", "value": {"shortDescription": [{"value": "kg", "lang": "en"}], "type": "unit group data set", "refObjectId": "ad38d542-3fe9-439d-9b95-2f5f7752acaf", "uri": "../unitgroups/ad38d542-3fe9-439d-9b95-2f5f7752acaf.xml"}}, {"value": "0", "module": "A1-A3"}, {"value": "0", "module": "A4"}, {"value": "0", "module": "A5"}, {"value": "0", "module": "C1"}, {"value": "0", "module": "C2", "scenario": "S1"}, {"value": "0", "module": "C2", "scenario": "S2"}, {"value": "0", "module": "C3", "scenario": "S1"}, {"value": "0", "module": "C3", "scenario": "S2"}, {"value": "0", "module": "D", "scenario": "S1"}, {"value": "0", "module": "D", "scenario": "S2"}]}, "resolvedFlowVersion": "38.00.000", "flowProperties": [], "typeOfFlow": "Other flow", "classification": {"classHierarchy": "Quantities / Environmental quantities / EPD EN 15804 / LCI indicators", "name": "GaBiCategories"}}, {"dataSetInternalID": 15, "referenceToFlowDataSet": {"shortDescription": [{"value": "Materials for recycling (MFR)", "lang": "en"}, {"value": "Stoffe zum Recycling (MFR)", "lang": "de"}], "type": "flow data set", "refObjectId": "d7fe48a5-4103-49c8-9aae-b0b5dfdbd6ae", "uri": "../flows/d7fe48a5-4103-49c8-9aae-b0b5dfdbd6ae.xml"}, "exchange direction": "OUTPUT", "other": {"anies": [{"name": "referenceToUnitGroupDataSet", "value": {"shortDescription": [{"value": "kg", "lang": "en"}], "type": "unit group data set", "refObjectId": "ad38d542-3fe9-439d-9b95-2f5f7752acaf", "uri": "../unitgroups/ad38d542-3fe9-439d-9b95-2f5f7752acaf.xml"}}, {"value": "0", "module": "A1-A3"}, {"value": "0", "module": "A4"}, {"value": "0.0988", "module": "A5"}, {"value": "0", "module": "C1"}, {"value": "0", "module": "C2", "scenario": "S1"}, {"value": "0", "module": "C2", "scenario": "S2"}, {"value": "1.65", "module": "C3", "scenario": "S1"}, {"value": "0", "module": "C3", "scenario": "S2"}, {"value": "0", "module": "D", "scenario": "S1"}, {"value": "0", "module": "D", "scenario": "S2"}]}, "resolvedFlowVersion": "38.00.000", "flowProperties": [], "typeOfFlow": "Other flow", "classification": {"classHierarchy": "Quantities / Environmental quantities / EPD EN 15804 / LCI indicators", "name": "GaBiCategories"}}, {"dataSetInternalID": 16, "referenceToFlowDataSet": {"shortDescription": [{"value": "Materials for energy recovery (MER)", "lang": "en"}, {"value": "Stoffe für die Energierückgewinnung (MER)", "lang": "de"}], "type": "flow data set", "refObjectId": "59a9181c-3aaf-46ee-8b13-2b3723b6e447", "uri": "../flows/59a9181c-3aaf-46ee-8b13-2b3723b6e447.xml"}, "exchange direction": "OUTPUT", "other": {"anies": [{"name": "referenceToUnitGroupDataSet", "value": {"shortDescription": [{"value": "kg", "lang": "en"}], "type": "unit group data set", "refObjectId": "ad38d542-3fe9-439d-9b95-2f5f7752acaf", "uri": "../unitgroups/ad38d542-3fe9-439d-9b95-2f5f7752acaf.xml"}}, {"value": "0", "module": "A1-A3"}, {"value": "0", "module": "A4"}, {"value": "0", "module": "A5"}, {"value": "0", "module": "C1"}, {"value": "0", "module": "C2", "scenario": "S1"}, {"value": "0", "module": "C2", "scenario": "S2"}, {"value": "0", "module": "C3", "scenario": "S1"}, {"value": "0", "module": "C3", "scenario": "S2"}, {"value": "0", "module": "D", "scenario": "S1"}, {"value": "0", "module": "D", "scenario": "S2"}]}, "resolvedFlowVersion": "38.00.000", "flowProperties": [], "typeOfFlow": "Other flow", "classification": {"classHierarchy": "Quantities / Environmental quantities / EPD EN 15804 / LCI indicators", "name": "GaBiCategories"}}, {"dataSetInternalID": 17, "referenceToFlowDataSet": {"shortDescription": [{"value": "Exported electrical energy (EEE)", "lang": "en"}, {"value": "Exportierte elektrische Energie (EEE)", "lang": "de"}], "type": "flow data set", "refObjectId": "4da0c987-2b76-40d6-9e9e-82a017aaaf29", "uri": "../flows/4da0c987-2b76-40d6-9e9e-82a017aaaf29.xml"}, "exchange direction": "OUTPUT", "other": {"anies": [{"name": "referenceToUnitGroupDataSet", "value": {"shortDescription": [{"value": "MJ", "lang": "en"}], "type": "unit group data set", "refObjectId": "93a60a57-a3c8-11da-a746-0800200c9a66", "uri": "../unitgroups/93a60a57-a3c8-11da-a746-0800200c9a66.xml"}}, {"value": "0", "module": "A1-A3"}, {"value": "0", "module": "A4"}, {"value": "0.846", "module": "A5"}, {"value": "0", "module": "C1"}, {"value": "0", "module": "C2", "scenario": "S1"}, {"value": "0", "module": "C2", "scenario": "S2"}, {"value": "0", "module": "C3", "scenario": "S1"}, {"value": "4.28", "module": "C3", "scenario": "S2"}, {"value": "0", "module": "D", "scenario": "S1"}, {"value": "0", "module": "D", "scenario": "S2"}]}, "resolvedFlowVersion": "38.00.000", "flowProperties": [], "typeOfFlow": "Other flow", "classification": {"classHierarchy": "Quantities / Environmental quantities / EPD EN 15804 / LCI indicators", "name": "GaBiCategories"}}, {"dataSetInternalID": 18, "referenceToFlowDataSet": {"shortDescription": [{"value": "Exported thermal energy (EET)", "lang": "en"}, {"value": "Exportierte thermische Energie (EET)", "lang": "de"}], "type": "flow data set", "refObjectId": "98daf38a-7a79-46d3-9a37-2b7bd0955810", "uri": "../flows/98daf38a-7a79-46d3-9a37-2b7bd0955810.xml"}, "exchange direction": "OUTPUT", "other": {"anies": [{"name": "referenceToUnitGroupDataSet", "value": {"shortDescription": [{"value": "MJ", "lang": "en"}], "type": "unit group data set", "refObjectId": "93a60a57-a3c8-11da-a746-0800200c9a66", "uri": "../unitgroups/93a60a57-a3c8-11da-a746-0800200c9a66.xml"}}, {"value": "0", "module": "A1-A3"}, {"value": "0", "module": "A4"}, {"value": "1.96", "module": "A5"}, {"value": "0", "module": "C1"}, {"value": "0", "module": "C2", "scenario": "S1"}, {"value": "0", "module": "C2", "scenario": "S2"}, {"value": "0", "module": "C3", "scenario": "S1"}, {"value": "7.77", "module": "C3", "scenario": "S2"}, {"value": "0", "module": "D", "scenario": "S1"}, {"value": "0", "module": "D", "scenario": "S2"}]}, "resolvedFlowVersion": "38.00.000", "flowProperties": [], "typeOfFlow": "Other flow", "classification": {"classHierarchy": "Quantities / Environmental quantities / EPD EN 15804 / LCI indicators", "name": "GaBiCategories"}}]}, "LCIAResults": {"LCIAResult": [{"referenceToLCIAMethodDataSet": {"shortDescription": [{"value": "Global Warming Potential total (GWP-total)", "lang": "en"}, {"value": "Globales Erwärmungspotenzial total (GWP-total)", "lang": "de"}], "type": "LCIA method data set", "refObjectId": "6a37f984-a4b3-458a-a20a-64418c145fa2", "uri": "../lciamethods/6a37f984-a4b3-458a-a20a-64418c145fa2.xml"}, "other": {"anies": [{"name": "referenceToUnitGroupDataSet", "value": {"shortDescription": [{"value": "kg CO_(2) eq", "lang": "en"}], "type": "unit group data set", "refObjectId": "1ebf3012-d0db-4de2-aefd-ef30cedb0be1", "uri": "../unitgroups/1ebf3012-d0db-4de2-aefd-ef30cedb0be1.xml"}}, {"value": "4.5856", "module": "A1-A3"}, {"value": "0.235", "module": "A4"}, {"value": "0.87", "module": "A5"}, {"value": "0", "module": "C1"}, {"value": "0.0127", "module": "C2", "scenario": "S1"}, {"value": "0.0127", "module": "C2", "scenario": "S2"}, {"value": "0.454", "module": "C3", "scenario": "S1"}, {"value": "3.22", "module": "C3", "scenario": "S2"}, {"value": "-3.08", "module": "D", "scenario": "S1"}, {"value": "-1.11", "module": "D", "scenario": "S2"}]}}, {"referenceToLCIAMethodDataSet": {"shortDescription": [{"value": "Global Warming Potential fossil fuels (GWP-fossil)", "lang": "en"}, {"value": "Globales Erwärmungspotenzial fossil (GWP-fossil)", "lang": "de"}], "type": "LCIA method data set", "refObjectId": "5f635281-343e-44fb-83df-1971b155e6b6", "uri": "../lciamethods/5f635281-343e-44fb-83df-1971b155e6b6.xml"}, "other": {"anies": [{"name": "referenceToUnitGroupDataSet", "value": {"shortDescription": [{"value": "kg CO_(2) eq", "lang": "en"}], "type": "unit group data set", "refObjectId": "1ebf3012-d0db-4de2-aefd-ef30cedb0be1", "uri": "../unitgroups/1ebf3012-d0db-4de2-aefd-ef30cedb0be1.xml"}}, {"value": "4.6206", "module": "A1-A3"}, {"value": "0.232", "module": "A4"}, {"value": "0.872", "module": "A5"}, {"value": "0", "module": "C1"}, {"value": "0.0124", "module": "C2", "scenario": "S1"}, {"value": "0.0124", "module": "C2", "scenario": "S2"}, {"value": "0.451", "module": "C3", "scenario": "S1"}, {"value": "3.22", "module": "C3", "scenario": "S2"}, {"value": "-3.06", "module": "D", "scenario": "S1"}, {"value": "-1.11", "module": "D", "scenario": "S2"}]}}, {"referenceToLCIAMethodDataSet": {"shortDescription": [{"value": "Global Warming Potential biogenic (GWP-biogenic)", "lang": "en"}, {"value": "Globales Erwärmungspotenzial biogen (GWP-biogenic)", "lang": "de"}], "type": "LCIA method data set", "refObjectId": "2356e1ab-0185-4db5-86e5-16de51c7485c", "uri": "../lciamethods/2356e1ab-0185-4db5-86e5-16de51c7485c.xml"}, "other": {"anies": [{"name": "referenceToUnitGroupDataSet", "value": {"shortDescription": [{"value": "kg CO_(2) eq", "lang": "en"}], "type": "unit group data set", "refObjectId": "1ebf3012-d0db-4de2-aefd-ef30cedb0be1", "uri": "../unitgroups/1ebf3012-d0db-4de2-aefd-ef30cedb0be1.xml"}}, {"value": "-0.03590331", "module": "A1-A3"}, {"value": "0.000663", "module": "A4"}, {"value": "-0.00191", "module": "A5"}, {"value": "0", "module": "C1"}, {"value": "7.09E-05", "module": "C2", "scenario": "S1"}, {"value": "7.09E-05", "module": "C2", "scenario": "S2"}, {"value": "0.00305", "module": "C3", "scenario": "S1"}, {"value": "-0.00026", "module": "C3", "scenario": "S2"}, {"value": "-0.0142", "module": "D", "scenario": "S1"}, {"value": "-0.00472", "module": "D", "scenario": "S2"}]}}, {"referenceToLCIAMethodDataSet": {"shortDescription": [{"value": "Global Warming Potential luluc (GWP-luluc)", "lang": "en"}, {"value": "Globales Erwärmungspotenzial luluc (GWP-luluc)", "lang": "de"}], "type": "LCIA method data set", "refObjectId": "4331bbdb-978a-490d-8707-eeb047f01a55", "uri": "../lciamethods/4331bbdb-978a-490d-8707-eeb047f01a55.xml"}, "other": {"anies": [{"name": "referenceToUnitGroupDataSet", "value": {"shortDescription": [{"value": "kg CO_(2) eq", "lang": "en"}], "type": "unit group data set", "refObjectId": "1ebf3012-d0db-4de2-aefd-ef30cedb0be1", "uri": "../unitgroups/1ebf3012-d0db-4de2-aefd-ef30cedb0be1.xml"}}, {"value": "0.0016345", "module": "A1-A3"}, {"value": "0.00222", "module": "A4"}, {"value": "0.00028", "module": "A5"}, {"value": "0", "module": "C1"}, {"value": "0.000238", "module": "C2", "scenario": "S1"}, {"value": "0.000238", "module": "C2", "scenario": "S2"}, {"value": "7.68E-05", "module": "C3", "scenario": "S1"}, {"value": "0.000717", "module": "C3", "scenario": "S2"}, {"value": "-0.00118", "module": "D", "scenario": "S1"}, {"value": "-9.96E-05", "module": "D", "scenario": "S2"}]}}, {"referenceToLCIAMethodDataSet": {"shortDescription": [{"value": "Depletion potential of the stratospheric ozone layer (ODP)", "lang": "en"}, {"value": "Abbau Potential der stratosphärischen Ozonschicht (ODP)", "lang": "de"}], "type": "LCIA method data set", "refObjectId": "b5c629d6-def3-11e6-bf01-fe55135034f3", "uri": "../lciamethods/b5c629d6-def3-11e6-bf01-fe55135034f3.xml"}, "other": {"anies": [{"name": "referenceToUnitGroupDataSet", "value": {"shortDescription": [{"value": "kg CFC11 eq", "lang": "en"}], "type": "unit group data set", "refObjectId": "d9e957c9-7309-4474-bf3a-7777df6c4e5b", "uri": "../unitgroups/d9e957c9-7309-4474-bf3a-7777df6c4e5b.xml"}}, {"value": "5.22535E-12", "module": "A1-A3"}, {"value": "5.05E-14", "module": "A4"}, {"value": "9.11E-13", "module": "A5"}, {"value": "0", "module": "C1"}, {"value": "3.91E-15", "module": "C2", "scenario": "S1"}, {"value": "3.91E-15", "module": "C2", "scenario": "S2"}, {"value": "5.96E-12", "module": "C3", "scenario": "S1"}, {"value": "2.48E-12", "module": "C3", "scenario": "S2"}, {"value": "-7.1E-12", "module": "D", "scenario": "S1"}, {"value": "-9.67E-12", "module": "D", "scenario": "S2"}]}}, {"referenceToLCIAMethodDataSet": {"shortDescription": [{"value": "Acidification potential of land and water (AP)", "lang": "en"}, {"value": "Versauerungspotenzial von Boden und Wasser (AP)", "lang": "de"}], "type": "LCIA method data set", "refObjectId": "b5c611c6-def3-11e6-bf01-fe55135034f3", "uri": "../lciamethods/b5c611c6-def3-11e6-bf01-fe55135034f3.xml"}, "other": {"anies": [{"name": "referenceToUnitGroupDataSet", "value": {"shortDescription": [{"value": "mol H^(+) eq", "lang": "en"}], "type": "unit group data set", "refObjectId": "42e089ac-92bf-4bf2-8ca1-5fc40d18f2ed", "uri": "../unitgroups/42e089ac-92bf-4bf2-8ca1-5fc40d18f2ed.xml"}}, {"value": "0.0120414", "module": "A1-A3"}, {"value": "0.00212", "module": "A4"}, {"value": "0.00098", "module": "A5"}, {"value": "0", "module": "C1"}, {"value": "1.23E-05", "module": "C2", "scenario": "S1"}, {"value": "1.23E-05", "module": "C2", "scenario": "S2"}, {"value": "0.000618", "module": "C3", "scenario": "S1"}, {"value": "0.000723", "module": "C3", "scenario": "S2"}, {"value": "-0.00468", "module": "D", "scenario": "S1"}, {"value": "-0.00115", "module": "D", "scenario": "S2"}]}}, {"referenceToLCIAMethodDataSet": {"shortDescription": [{"value": "Eutrophication potential aquatic freshwater (EP-freshwater)", "lang": "en"}, {"value": "Eutrophierungspotenzial Süßwasser (EP-freshwater)", "lang": "de"}], "type": "LCIA method data set", "refObjectId": "b53ec18f-7377-4ad3-86eb-cc3f4f276b2b", "uri": "../lciamethods/b53ec18f-7377-4ad3-86eb-cc3f4f276b2b.xml"}, "other": {"anies": [{"name": "referenceToUnitGroupDataSet", "value": {"shortDescription": [{"value": "kg P eq", "lang": "en"}], "type": "unit group data set", "refObjectId": "0429039d-a61d-4590-ba67-aa4a20a810a1", "uri": "../unitgroups/0429039d-a61d-4590-ba67-aa4a20a810a1.xml"}}, {"value": "2.0087E-05", "module": "A1-A3"}, {"value": "3.42E-07", "module": "A4"}, {"value": "1.54E-06", "module": "A5"}, {"value": "0", "module": "C1"}, {"value": "3.37E-08", "module": "C2", "scenario": "S1"}, {"value": "3.37E-08", "module": "C2", "scenario": "S2"}, {"value": "4.49E-06", "module": "C3", "scenario": "S1"}, {"value": "6.62E-07", "module": "C3", "scenario": "S2"}, {"value": "-3.74E-06", "module": "D", "scenario": "S1"}, {"value": "-1.81E-06", "module": "D", "scenario": "S2"}]}}, {"referenceToLCIAMethodDataSet": {"shortDescription": [{"value": "Eutrophication potential aquatic marine (EP-marine)", "lang": "en"}, {"value": "Eutrophierungspotenzial Salzwasser (EP-marine)", "lang": "de"}], "type": "LCIA method data set", "refObjectId": "b5c619fa-def3-11e6-bf01-fe55135034f3", "uri": "../lciamethods/b5c619fa-def3-11e6-bf01-fe55135034f3.xml"}, "other": {"anies": [{"name": "referenceToUnitGroupDataSet", "value": {"shortDescription": [{"value": "kg N eq", "lang": "en"}], "type": "unit group data set", "refObjectId": "d05bb823-ecdf-4686-8c40-bf1d9257859f", "uri": "../unitgroups/d05bb823-ecdf-4686-8c40-bf1d9257859f.xml"}}, {"value": "0.00283656", "module": "A1-A3"}, {"value": "0.000951", "module": "A4"}, {"value": "0.000257", "module": "A5"}, {"value": "0", "module": "C1"}, {"value": "3.67E-06", "module": "C2", "scenario": "S1"}, {"value": "3.67E-06", "module": "C2", "scenario": "S2"}, {"value": "0.000164", "module": "C3", "scenario": "S1"}, {"value": "0.000236", "module": "C3", "scenario": "S2"}, {"value": "-0.00135", "module": "D", "scenario": "S1"}, {"value": "-0.000352", "module": "D", "scenario": "S2"}]}}, {"referenceToLCIAMethodDataSet": {"shortDescription": [{"value": "Eutrophication potential terrestrial (EP-terrestrial)", "lang": "en"}, {"value": "Eutrophierungspotenzial Land (EP-terrestrial)", "lang": "de"}], "type": "LCIA method data set", "refObjectId": "b5c614d2-def3-11e6-bf01-fe55135034f3", "uri": "../lciamethods/b5c614d2-def3-11e6-bf01-fe55135034f3.xml"}, "other": {"anies": [{"name": "referenceToUnitGroupDataSet", "value": {"shortDescription": [{"value": "mol N eq", "lang": "en"}], "type": "unit group data set", "refObjectId": "71b4d617-0ec9-4d3f-b65e-e438940c2401", "uri": "../unitgroups/71b4d617-0ec9-4d3f-b65e-e438940c2401.xml"}}, {"value": "0.032793", "module": "A1-A3"}, {"value": "0.0105", "module": "A4"}, {"value": "0.00312", "module": "A5"}, {"value": "0", "module": "C1"}, {"value": "4.71E-05", "module": "C2", "scenario": "S1"}, {"value": "4.71E-05", "module": "C2", "scenario": "S2"}, {"value": "0.00172", "module": "C3", "scenario": "S1"}, {"value": "0.00312", "module": "C3", "scenario": "S2"}, {"value": "-0.0144", "module": "D", "scenario": "S1"}, {"value": "-0.00378", "module": "D", "scenario": "S2"}]}}, {"referenceToLCIAMethodDataSet": {"shortDescription": [{"value": "Formation potential of tropospheric ozone photochemical oxidants (POCP)", "lang": "en"}, {"value": "Bildungspotential für troposphärisches Ozon (POCP)", "lang": "de"}], "type": "LCIA method data set", "refObjectId": "b5c610fe-def3-11e6-bf01-fe55135034f3", "uri": "../lciamethods/b5c610fe-def3-11e6-bf01-fe55135034f3.xml"}, "other": {"anies": [{"name": "referenceToUnitGroupDataSet", "value": {"shortDescription": [{"value": "kg NMVOC eq", "lang": "en"}], "type": "unit group data set", "refObjectId": "d27c25f8-fbc1-44c6-b47b-4adbae4199c6", "uri": "../unitgroups/d27c25f8-fbc1-44c6-b47b-4adbae4199c6.xml"}}, {"value": "0.0094551", "module": "A1-A3"}, {"value": "0.0026", "module": "A4"}, {"value": "0.000806", "module": "A5"}, {"value": "0", "module": "C1"}, {"value": "1.2E-05", "module": "C2", "scenario": "S1"}, {"value": "1.2E-05", "module": "C2", "scenario": "S2"}, {"value": "0.000437", "module": "C3", "scenario": "S1"}, {"value": "0.000679", "module": "C3", "scenario": "S2"}, {"value": "-0.00642", "module": "D", "scenario": "S1"}, {"value": "-0.000998", "module": "D", "scenario": "S2"}]}}, {"referenceToLCIAMethodDataSet": {"shortDescription": [{"value": "Abiotic depletion potential for non fossil resources (ADPE)", "lang": "en"}, {"value": "Potenzial für den abiotischen Abbau nicht fossiler Ressourcen (ADPE)", "lang": "de"}], "type": "LCIA method data set", "refObjectId": "b2ad6494-c78d-11e6-9d9d-cec0c932ce01", "uri": "../lciamethods/b2ad6494-c78d-11e6-9d9d-cec0c932ce01.xml"}, "other": {"anies": [{"name": "referenceToUnitGroupDataSet", "value": {"shortDescription": [{"value": "kg Sb eq", "lang": "en"}], "type": "unit group data set", "refObjectId": "54ccd2d9-a32a-4fc2-923d-f2c8c93e89d4", "uri": "../unitgroups/54ccd2d9-a32a-4fc2-923d-f2c8c93e89d4.xml"}}, {"value": "1.75048E-06", "module": "A1-A3"}, {"value": "3.34E-08", "module": "A4"}, {"value": "1.16E-07", "module": "A5"}, {"value": "0", "module": "C1"}, {"value": "2.11E-09", "module": "C2", "scenario": "S1"}, {"value": "2.11E-09", "module": "C2", "scenario": "S2"}, {"value": "1.03E-07", "module": "C3", "scenario": "S1"}, {"value": "2.59E-08", "module": "C3", "scenario": "S2"}, {"value": "-2.27E-07", "module": "D", "scenario": "S1"}, {"value": "-9.46E-08", "module": "D", "scenario": "S2"}]}}, {"referenceToLCIAMethodDataSet": {"shortDescription": [{"value": "Abiotic depletion potential for fossil resources (ADPF)", "lang": "en"}, {"value": "Potenzial für den abiotischen Abbau fossiler Brennstoffe (ADPF)", "lang": "de"}], "type": "LCIA method data set", "refObjectId": "b2ad6110-c78d-11e6-9d9d-cec0c932ce01", "uri": "../lciamethods/b2ad6110-c78d-11e6-9d9d-cec0c932ce01.xml"}, "other": {"anies": [{"name": "referenceToUnitGroupDataSet", "value": {"shortDescription": [{"value": "MJ", "lang": "en"}], "type": "unit group data set", "refObjectId": "93a60a57-a3c8-11da-a746-0800200c9a66", "uri": "../unitgroups/93a60a57-a3c8-11da-a746-0800200c9a66.xml"}}, {"value": "114.409", "module": "A1-A3"}, {"value": "2.92", "module": "A4"}, {"value": "7.74", "module": "A5"}, {"value": "0", "module": "C1"}, {"value": "0.163", "module": "C2", "scenario": "S1"}, {"value": "0.163", "module": "C2", "scenario": "S2"}, {"value": "6.34", "module": "C3", "scenario": "S1"}, {"value": "5.04", "module": "C3", "scenario": "S2"}, {"value": "-106", "module": "D", "scenario": "S1"}, {"value": "-19.7", "module": "D", "scenario": "S2"}]}}, {"referenceToLCIAMethodDataSet": {"shortDescription": [{"value": "Water use (WDP)", "lang": "en"}, {"value": "Wassernutzung (WDP)", "lang": "de"}], "type": "LCIA method data set", "refObjectId": "b2ad66ce-c78d-11e6-9d9d-cec0c932ce01", "uri": "../lciamethods/b2ad66ce-c78d-11e6-9d9d-cec0c932ce01.xml"}, "other": {"anies": [{"name": "referenceToUnitGroupDataSet", "value": {"shortDescription": [{"value": "m^(3) world eq deprived", "lang": "en"}], "type": "unit group data set", "refObjectId": "6ae2df01-888e-46c8-b17d-49fa3869b476", "uri": "../unitgroups/6ae2df01-888e-46c8-b17d-49fa3869b476.xml"}}, {"value": "2.61757", "module": "A1-A3"}, {"value": "0.00132", "module": "A4"}, {"value": "0.214", "module": "A5"}, {"value": "0", "module": "C1"}, {"value": "8.88E-05", "module": "C2", "scenario": "S1"}, {"value": "8.88E-05", "module": "C2", "scenario": "S2"}, {"value": "0.0896", "module": "C3", "scenario": "S1"}, {"value": "0.32", "module": "C3", "scenario": "S2"}, {"value": "-0.253", "module": "D", "scenario": "S1"}, {"value": "-0.118", "module": "D", "scenario": "S2"}]}}, {"referenceToLCIAMethodDataSet": {"shortDescription": [{"value": "Incidence of disease due to PM emissions (PM)", "lang": "en"}, {"value": "Auftreten von Krankheiten aufgrund von Feinstaubemissionen (PM)", "lang": "de"}], "type": "LCIA method data set", "refObjectId": "b5c602c6-def3-11e6-bf01-fe55135034f3", "uri": "../lciamethods/b5c602c6-def3-11e6-bf01-fe55135034f3.xml"}, "other": {"anies": [{"name": "referenceToUnitGroupDataSet", "value": {"shortDescription": [{"value": "Disease incidence", "lang": "en"}], "type": "unit group data set", "refObjectId": "3883559b-648f-4afc-8ba2-0bd24f3affa3", "uri": "../unitgroups/3883559b-648f-4afc-8ba2-0bd24f3affa3.xml"}}, {"value": "1.44855E-07", "module": "A1-A3"}, {"value": "5.76E-08", "module": "A4"}, {"value": "1.35E-08", "module": "A5"}, {"value": "0", "module": "C1"}, {"value": "1.3E-10", "module": "C2", "scenario": "S1"}, {"value": "1.3E-10", "module": "C2", "scenario": "S2"}, {"value": "5.27E-09", "module": "C3", "scenario": "S1"}, {"value": "1.62E-08", "module": "C3", "scenario": "S2"}, {"value": "-5.79E-08", "module": "D", "scenario": "S1"}, {"value": "-9.41E-09", "module": "D", "scenario": "S2"}]}}, {"referenceToLCIAMethodDataSet": {"shortDescription": [{"value": "Human exposure efficiency relative to U235 (IR)", "lang": "en"}, {"value": "Wirkung durch Exposition des Menschen mit U235 (IR)", "lang": "de"}], "type": "LCIA method data set", "refObjectId": "b5c632be-def3-11e6-bf01-fe55135034f3", "uri": "../lciamethods/b5c632be-def3-11e6-bf01-fe55135034f3.xml"}, "other": {"anies": [{"name": "referenceToUnitGroupDataSet", "value": {"shortDescription": [{"value": "kBq U235 eq", "lang": "en"}], "type": "unit group data set", "refObjectId": "456b05bf-1415-44a9-9993-02452f554c09", "uri": "../unitgroups/456b05bf-1415-44a9-9993-02452f554c09.xml"}}, {"value": "0.414622", "module": "A1-A3"}, {"value": "0.000579", "module": "A4"}, {"value": "0.0355", "module": "A5"}, {"value": "0", "module": "C1"}, {"value": "2.73E-05", "module": "C2", "scenario": "S1"}, {"value": "2.73E-05", "module": "C2", "scenario": "S2"}, {"value": "0.144", "module": "C3", "scenario": "S1"}, {"value": "0.0159", "module": "C3", "scenario": "S2"}, {"value": "-0.116", "module": "D", "scenario": "S1"}, {"value": "-0.236", "module": "D", "scenario": "S2"}]}}, {"referenceToLCIAMethodDataSet": {"shortDescription": [{"value": "Comparative toxic unit for ecosystems (ETP-fw)", "lang": "en"}, {"value": "Toxizitätsvergleichseinheit für Ökosysteme (ETP-fw)", "lang": "de"}], "type": "LCIA method data set", "refObjectId": "ee1082d1-b0f7-43ca-a1f0-21e2a4a74511", "uri": "../lciamethods/ee1082d1-b0f7-43ca-a1f0-21e2a4a74511.xml"}, "other": {"anies": [{"name": "referenceToUnitGroupDataSet", "value": {"shortDescription": [{"value": "CTUe", "lang": "en"}], "type": "unit group data set", "refObjectId": "aa959ded-f1eb-4efb-9c5c-2d60be36b3e6", "uri": "../unitgroups/aa959ded-f1eb-4efb-9c5c-2d60be36b3e6.xml"}}, {"value": "53.634", "module": "A1-A3"}, {"value": "2.27", "module": "A4"}, {"value": "3.54", "module": "A5"}, {"value": "0", "module": "C1"}, {"value": "0.126", "module": "C2", "scenario": "S1"}, {"value": "0.126", "module": "C2", "scenario": "S2"}, {"value": "1.96", "module": "C3", "scenario": "S1"}, {"value": "3.8", "module": "C3", "scenario": "S2"}, {"value": "-55.8", "module": "D", "scenario": "S1"}, {"value": "-2.74", "module": "D", "scenario": "S2"}]}}, {"referenceToLCIAMethodDataSet": {"shortDescription": [{"value": "Comparative toxic unit for humans (carcinogenic) (HTP-c)", "lang": "en"}, {"value": "Toxizitätsvergleichseinheit für Menschen (krebserregend) (HTP-c)", "lang": "de"}], "type": "LCIA method data set", "refObjectId": "2299222a-bbd8-474f-9d4f-4dd1f18aea7c", "uri": "../lciamethods/2299222a-bbd8-474f-9d4f-4dd1f18aea7c.xml"}, "other": {"anies": [{"name": "referenceToUnitGroupDataSet", "value": {"shortDescription": [{"value": "CTUh", "lang": "en"}], "type": "unit group data set", "refObjectId": "d4c9523e-2d7e-49fd-8469-998f547d3a70", "uri": "../unitgroups/d4c9523e-2d7e-49fd-8469-998f547d3a70.xml"}}, {"value": "1.192889E-08", "module": "A1-A3"}, {"value": "4.14E-11", "module": "A4"}, {"value": "7.34E-10", "module": "A5"}, {"value": "0", "module": "C1"}, {"value": "2.52E-12", "module": "C2", "scenario": "S1"}, {"value": "2.52E-12", "module": "C2", "scenario": "S2"}, {"value": "1.03E-10", "module": "C3", "scenario": "S1"}, {"value": "1.25E-10", "module": "C3", "scenario": "S2"}, {"value": "-1.27E-09", "module": "D", "scenario": "S1"}, {"value": "-2.24E-10", "module": "D", "scenario": "S2"}]}}, {"referenceToLCIAMethodDataSet": {"shortDescription": [{"value": "Comparative toxic unit for humans (noncarcinogenic) (HTP-nc)", "lang": "en"}, {"value": "Toxizitätsvergleichseinheit für Menschen (nicht krebserregend) (HTP-nc)", "lang": "de"}], "type": "LCIA method data set", "refObjectId": "3af763a5-b7a1-48c9-9cee-1f223481fcef", "uri": "../lciamethods/3af763a5-b7a1-48c9-9cee-1f223481fcef.xml"}, "other": {"anies": [{"name": "referenceToUnitGroupDataSet", "value": {"shortDescription": [{"value": "CTUh", "lang": "en"}], "type": "unit group data set", "refObjectId": "d4c9523e-2d7e-49fd-8469-998f547d3a70", "uri": "../unitgroups/d4c9523e-2d7e-49fd-8469-998f547d3a70.xml"}}, {"value": "2.35927E-07", "module": "A1-A3"}, {"value": "1.33E-09", "module": "A4"}, {"value": "1.5E-08", "module": "A5"}, {"value": "0", "module": "C1"}, {"value": "1.06E-10", "module": "C2", "scenario": "S1"}, {"value": "1.06E-10", "module": "C2", "scenario": "S2"}, {"value": "2.19E-09", "module": "C3", "scenario": "S1"}, {"value": "9.93E-09", "module": "C3", "scenario": "S2"}, {"value": "-4.52E-08", "module": "D", "scenario": "S1"}, {"value": "-5.3E-09", "module": "D", "scenario": "S2"}]}}, {"referenceToLCIAMethodDataSet": {"shortDescription": [{"value": "Soil quality index (SQP)", "lang": "en"}, {"value": "Bodenqualitätsindex (SQP)", "lang": "de"}], "type": "LCIA method data set", "refObjectId": "b2ad6890-c78d-11e6-9d9d-cec0c932ce01", "uri": "../lciamethods/b2ad6890-c78d-11e6-9d9d-cec0c932ce01.xml"}, "other": {"anies": [{"name": "referenceToUnitGroupDataSet", "value": {"shortDescription": [{"value": "SQP", "lang": "en"}], "type": "unit group data set", "refObjectId": "f130951c-e67f-4f7f-8dd4-665de3974e18", "uri": "../unitgroups/f130951c-e67f-4f7f-8dd4-665de3974e18.xml"}}, {"value": "5.5131", "module": "A1-A3"}, {"value": "1.01", "module": "A4"}, {"value": "0.644", "module": "A5"}, {"value": "0", "module": "C1"}, {"value": "0.108", "module": "C2", "scenario": "S1"}, {"value": "0.108", "module": "C2", "scenario": "S2"}, {"value": "2.38", "module": "C3", "scenario": "S1"}, {"value": "1.23", "module": "C3", "scenario": "S2"}, {"value": "-3.04", "module": "D", "scenario": "S1"}, {"value": "-3.79", "module": "D", "scenario": "S2"}]}}]}, "otherAttributes": {"{http://www.indata.network/EPD/2019}epd-version": "1.2"}, "version": "1.1", "locations": "../ILCDLocations.xml"}