{"processInformation": {"dataSetInformation": {"UUID": "b40945b8-3dad-45e7-8edb-64533906f724", "name": {"baseName": [{"value": "SANHA®-Press | Copper Press Fittings", "lang": "en"}]}, "classificationInformation": {"classification": [{"class": [{"value": "Metalle", "level": 0, "classId": "4"}, {"value": "Kupfer", "level": 1, "classId": "4.4"}, {"value": "Kupferrohre", "level": 2, "classId": "4.4.02"}], "name": "OEKOBAU.DAT"}]}, "generalComment": [{"value": "The owner of this EPD shall be liable for the underlying information and evidence. The programme operator Kiwa-Ecobility Experts shall not be liable with respect to manufacturer data, life cycle assessment data and evidence.", "lang": "en"}], "other": {"anies": [{"scenario": [{"description": [{"value": "We assume that demolition of the plant consumes very little energy and therefore falls under the cut of rules (<1%)."}], "name": "Standard scenario", "default": true}]}]}}, "quantitativeReference": {"referenceToReferenceFlow": [1], "type": "Reference flow(s)"}, "time": {"referenceYear": 2023, "dataSetValidUntil": 2029, "timeRepresentativenessDescription": [{"value": "Data collection of the used raw materials, suppliers information, energy consumption, production waste and emissions are all based on the reference year 2023. ", "lang": "en"}], "other": {"anies": [{"name": "publicationDateOfEPD", "value": 1722470400000}]}}, "geography": {"locationOfOperationSupplyOrProduction": {"descriptionOfRestrictions": [{"value": "The results of this EPD are representative for European Union. ", "lang": "en"}], "location": "EU-27"}}, "technology": {"technologyDescriptionAndIncludedProcesses": [{"value": "The SANHA®-Press system fittings are made of copper, CU-DHP (material number CW024A). The SANHA®-Press system meets the highest quality standards, can be easily installed and provides a solution for a large number of applications. The system ensures a permanent leak-proof connection by compressing the fitting perpendicular onto the pipe. The pressing procedure deforms the pipe and fitting which creates a permanent leak-proof connection. The SANHA®-Press system can be ideally combined with our unique PURAPRESS® Series 8000 system (for which a separate environmental product declaration has been written) made of completely lead-free copper alloy silicon bronze or all standard copper pipes. The extensive range (12 mm – 108 mm) of the SANHA®-Press system pipes are suitable for equipping buildings with risers and horizontal lines. The weight of the SANHA®-Press system fittings can be various due to the different dimensions of the product. Features: 1. Unique tool compatibility = The SANHA®-Press system fittings can be pressed with press jaws and slings with the original SA, V and M-profiles up to and including 54 mm and up to 108 mm with SA and M profile. 2. Leak path feature = The SANHA®-Press system fittings benefit from a leak before press function. 3. Push & stay = The SANHA®-Press system fittings are designed in a way that safe and reliable installation in every position is guaranteed. The SANHA®-Press system fittings, which are manufactured in Ternat, Belgium,  are produced from copper tubes CU-DHP (material number CW024A) and are cold deformed. The cold deformation proces consists of multiple production steps depending on the type of fitting being produced. The raw material is always cut in the proper length. Here you can find an overview of the various cold deformation steps: Bending into the correct radius; Opening up the pipe ends; Forming the sealing ring groove; Calibration; Forming of tee pieces through hydroforming process; After the cold deformation process, the semi finished product is mounted with a specific sealing ring and afterwards packed in plastic bags and carton boxes. The energy used during the production phase is partially generated by solar panels. The other part of the energy consumed is green energy which is bought and stated in the Guarantee of Origin.", "lang": "en"}], "technologicalApplicability": [{"value": "For drinking water and heating installations, compressed air, rainwater, fire extinguishing systems, ship building, inert gases, cooling water (with glycol), flammable gasses, hydrogen and technical and industrial gasses. More applications can be requested on demand. Different seals are inserted into the fittings depending on the system: SANHA®-Press (Series 6000) | Copper: Sealing ring made of Ethyleen Propyleen Dieen Monomeer (EPDM); SANHA®-Press Gas (Series 10000/11000) | Copper: Sealing ring made of Hydrogenated Nitrile Butadiene Rubber (HNBR); SANHA®-Press Solar (Series 12000/13000) | Copper: Sealing ring made of fluoro rubber (FKM)", "lang": "en"}], "referenceToTechnologyFlowDiagrammOrPicture": [{"shortDescription": [{"value": "Flow chart SANHA®-Press | Copper Press Fittings", "lang": "en"}], "type": "source data set", "refObjectId": "78b61620-af9a-4f31-bb1a-20d931b49d85", "version": "00.00.001"}]}}, "modellingAndValidation": {"LCIMethodAndAllocation": {"typeOfDataSet": "EPD", "other": {"anies": [{"name": "subType", "value": "specific dataset"}]}}, "dataSourcesTreatmentAndRepresentativeness": {"referenceToDataSource": [{"shortDescription": [{"value": "ecoinvent 3.6 database", "lang": "en"}], "type": "source data set", "refObjectId": "766b9973-5ee8-48a2-8098-72c8e20b369f", "version": "00.00.001"}, {"shortDescription": [{"value": "ecoinvent database (general)", "lang": "en"}], "type": "source data set", "refObjectId": "b497a91f-e14b-4b69-8f28-f50eb1576766", "version": "00.03.002"}], "useAdviceForDataSet": [{"value": "For drinking water and heating installations, compressed air, rainwater, fire extinguishing systems, ship building, inert gases, cooling water (with glycol), flammable gasses, hydrogen and technical and industrial gasses. More applications can be requested on demand. Different seals are inserted into the fittings depending on the system: SANHA®-Press (Series 6000) | Copper: Sealing ring made of Ethyleen Propyleen Dieen Monomeer (EPDM); SANHA®-Press Gas (Series 10000/11000) | Copper: Sealing ring made of Hydrogenated Nitrile Butadiene Rubber (HNBR); SANHA®-Press Solar (Series 12000/13000) | Copper: Sealing ring made of fluoro rubber (FKM)", "lang": "en"}], "other": {"anies": [{"name": "referenceToOriginalEPD", "value": {"shortDescription": {"value": "SANHA®-Press | Copper Press Fittings EPD", "defaultValue": "SANHA®-Press | Copper Press Fittings EPD", "lstrings": [{"lang": "en", "value": "SANHA®-Press | Copper Press Fittings EPD"}]}, "version": {"version": 1, "majorVersion": 0, "minorVersion": 0, "subMinorVersion": 1, "zero": false, "versionString": "00.00.001"}, "type": "source data set", "uuid": {"uuid": "b6eeb459-a1e5-4c81-92b3-2b6da33e1dca"}, "refObjectId": "b6eeb459-a1e5-4c81-92b3-2b6da33e1dca", "versionAsString": "00.00.001", "resourceURLs": ["https://oekobaudat.de/OEKOBAU.DAT/resource/sources/b6eeb459-a1e5-4c81-92b3-2b6da33e1dca/EPD-Kiwa-EE-178231-EN.pdf?version=00.00.001"]}}]}}, "validation": {"review": [{"reviewDetails": [{"value": "The independent verification is in accordance with the ISO 14025:2011. ", "lang": "en"}], "referenceToNameOfReviewerAndInstitution": [{"shortDescription": [{"value": "Lucas Pedro Berman, Senda", "lang": "en"}], "type": "contact data set", "refObjectId": "2294137c-5a52-4a75-965f-770e74b24b10", "version": "00.00.002"}], "type": "Independent external review"}]}, "complianceDeclarations": {"compliance": [{"referenceToComplianceSystem": {"shortDescription": [{"value": "EN 15804+A2", "lang": "de"}, {"value": "EN 15804+A2", "lang": "en"}], "type": "source data set", "refObjectId": "c0016b33-8cf7-415c-ac6e-deba0d21440d", "version": "00.01.000"}}, {"referenceToComplianceSystem": {"shortDescription": [{"value": "ISO 14025", "lang": "en"}], "type": "source data set", "refObjectId": "4f2eb655-6e44-4874-a95a-e28f5442cd4d", "version": "00.00.001"}}]}}, "administrativeInformation": {"commissionerAndGoal": {"referenceToCommissioner": [{"shortDescription": [{"value": "SANHA GmbH & Co. KG", "lang": "en"}], "type": "contact data set", "refObjectId": "2985e03b-e8d5-483f-910e-15e98721a88c", "version": "00.00.001"}]}, "dataGenerator": {"referenceToPersonOrEntityGeneratingTheDataSet": [{"shortDescription": [{"value": "SANHA GmbH & Co. KG", "lang": "en"}], "type": "contact data set", "refObjectId": "2985e03b-e8d5-483f-910e-15e98721a88c", "version": "00.00.001"}]}, "dataEntryBy": {"timeStamp": 1724243000595, "referenceToDataSetFormat": [{"shortDescription": [{"value": "EPD Data Format Extensions v1.2", "lang": "en"}, {"value": "EPD-Datenformaterweiterungen v1.2", "lang": "de"}], "type": "source data set", "refObjectId": "a29449fd-aa2f-4de8-b5d7-4b06b43c6fde", "version": "00.01.000"}, {"shortDescription": [{"value": "ILCD format", "lang": "en"}], "type": "source data set", "refObjectId": "a97a0155-0234-4b87-b4ce-a45da52f2a40", "version": "01.00.001", "uri": "http://lca.jrc.ec.europa.eu/lcainfohub/sample_data/ilcd/sources/ILCD_Format_a97a0155-0234-4b87-b4ce-a45da52f2a40_01.00.000.xml"}], "referenceToPersonOrEntityEnteringTheData": {"shortDescription": [{"value": "Kiwa GmbH (Berlin)", "lang": "en"}], "type": "contact data set", "refObjectId": "3ea4a87a-3f88-4633-b7e7-1bbdd272be43", "version": "00.00.002"}}, "publicationAndOwnership": {"dataSetVersion": "00.00.009", "referenceToRegistrationAuthority": {"shortDescription": [{"value": "Kiwa-Ecobility Experts, Kiwa GmbH (Berlin)", "lang": "en"}], "type": "contact data set", "refObjectId": "eb52a9a8-9d0f-40ce-a5c9-7b78f5615e5a", "version": "00.00.002"}, "registrationNumber": "EPD-Kiwa-EE-178231-EN", "referenceToOwnershipOfDataSet": {"shortDescription": [{"value": "SANHA GmbH & Co. KG", "lang": "en"}], "type": "contact data set", "refObjectId": "2985e03b-e8d5-483f-910e-15e98721a88c", "version": "00.00.001"}, "copyright": true, "licenseType": "Free of charge for all users and uses", "accessRestrictions": [{"value": "None.", "lang": "en"}], "other": {"anies": [{"name": "referenceToPublisher", "value": {"shortDescription": [{"value": "Kiwa-Ecobility Experts, Kiwa GmbH (Berlin)", "lang": "en"}], "type": "contact data set", "refObjectId": "eb52a9a8-9d0f-40ce-a5c9-7b78f5615e5a", "version": "00.00.002"}}]}}}, "exchanges": {"exchange": [{"dataSetInternalID": 1, "referenceToFlowDataSet": {"shortDescription": [{"value": "SANHA®-Press | Copper Press Fittings", "lang": "en"}], "type": "flow data set", "refObjectId": "bbb41d44-f96b-4260-9573-afde478dd293", "version": "00.00.001"}, "meanAmount": 1.0, "resultingAmount": 1.0, "referenceFlow": true, "resultingflowAmount": 1.0, "flowProperties": [{"name": [{"lang": "en", "value": "Mass"}, {"lang": "de", "value": "Masse"}], "uuid": "93a60a56-a3c8-11da-a746-0800200b9a66", "referenceFlowProperty": true, "meanValue": 1.0, "referenceUnit": "kg", "unitGroupUUID": "ad38d542-3fe9-439d-9b95-2f5f7752acaf"}], "materialProperties": [{"name": "gross density", "value": "8940.0", "unit": "kg/m^3", "unitDescription": "kilograms per cubic metre"}], "typeOfFlow": "Product flow", "classification": {"classHierarchy": "Metalle / Kupfer / Kupferrohre", "name": "OEKOBAU.DAT"}}, {"dataSetInternalID": 2, "referenceToFlowDataSet": {"shortDescription": [{"value": "Komponenten für die Wiederverwendung (CRU)", "lang": "de"}, {"value": "Components for re-use (CRU)", "lang": "en"}, {"value": "Componentes para su reutilización (CRU)", "lang": "es"}, {"value": "Komponenter för återanvändning (CRU)", "lang": "sv"}], "type": "flow data set", "refObjectId": "a2b32f97-3fc7-4af2-b209-525bc6426f33", "version": "30.00.002"}, "exchange direction": "OUTPUT", "meanAmount": 0.0, "other": {"anies": [{"value": "0.0", "module": "A1", "scenario": "Standard scenario"}, {"value": "0.0", "module": "A2", "scenario": "Standard scenario"}, {"value": "0.0", "module": "A3", "scenario": "Standard scenario"}, {"value": "0.0", "module": "A4", "scenario": "Standard scenario"}, {"value": "0.00210021", "module": "A5", "scenario": "Standard scenario"}, {"value": "0.0", "module": "B1", "scenario": "Standard scenario"}, {"value": "0.0", "module": "B2", "scenario": "Standard scenario"}, {"value": "0.0", "module": "B3", "scenario": "Standard scenario"}, {"value": "0.0", "module": "B4", "scenario": "Standard scenario"}, {"value": "0.0", "module": "B5", "scenario": "Standard scenario"}, {"value": "0.0", "module": "B6", "scenario": "Standard scenario"}, {"value": "0.0", "module": "B7", "scenario": "Standard scenario"}, {"value": "0.0", "module": "C1", "scenario": "Standard scenario"}, {"value": "0.0", "module": "C2", "scenario": "Standard scenario"}, {"value": "0.0", "module": "C3", "scenario": "Standard scenario"}, {"value": "0.0", "module": "C4", "scenario": "Standard scenario"}, {"value": "0.0", "module": "D", "scenario": "Standard scenario"}, {"name": "referenceToUnitGroupDataSet", "value": {"shortDescription": [{"value": "kg"}], "type": "unit group data set", "refObjectId": "ad38d542-3fe9-439d-9b95-2f5f7752acaf", "uri": "../unitgroups/ad38d542-3fe9-439d-9b95-2f5f7752acaf"}}]}, "resolvedFlowVersion": "38.00.000", "flowProperties": [], "typeOfFlow": "Other flow", "classification": {"classHierarchy": "Quantities / Environmental quantities / EPD EN 15804 / LCI indicators", "name": "GaBiCategories"}}, {"dataSetInternalID": 3, "referenceToFlowDataSet": {"shortDescription": [{"value": "Exportierte elektrische Energie (EEE)", "lang": "de"}, {"value": "Exported electrical energy (EEE)", "lang": "en"}, {"value": "Energía exportada electrica (EEE)", "lang": "es"}, {"value": "Exporterad energi – elektrisk (EEE)", "lang": "sv"}], "type": "flow data set", "refObjectId": "4da0c987-2b76-40d6-9e9e-82a017aaaf29", "version": "30.00.002"}, "exchange direction": "OUTPUT", "meanAmount": 0.0, "other": {"anies": [{"value": "0.0", "module": "A1", "scenario": "Standard scenario"}, {"value": "0.0", "module": "A2", "scenario": "Standard scenario"}, {"value": "-0.0631221157394019", "module": "A3", "scenario": "Standard scenario"}, {"value": "0.0", "module": "A4", "scenario": "Standard scenario"}, {"value": "0.0", "module": "A5", "scenario": "Standard scenario"}, {"value": "0.0", "module": "B1", "scenario": "Standard scenario"}, {"value": "0.0", "module": "B2", "scenario": "Standard scenario"}, {"value": "0.0", "module": "B3", "scenario": "Standard scenario"}, {"value": "0.0", "module": "B4", "scenario": "Standard scenario"}, {"value": "0.0", "module": "B5", "scenario": "Standard scenario"}, {"value": "0.0", "module": "B6", "scenario": "Standard scenario"}, {"value": "0.0", "module": "B7", "scenario": "Standard scenario"}, {"value": "0.0", "module": "C1", "scenario": "Standard scenario"}, {"value": "0.0", "module": "C2", "scenario": "Standard scenario"}, {"value": "0.0", "module": "C3", "scenario": "Standard scenario"}, {"value": "0.0", "module": "C4", "scenario": "Standard scenario"}, {"value": "-0.143702866130143", "module": "D", "scenario": "Standard scenario"}, {"name": "referenceToUnitGroupDataSet", "value": {"shortDescription": [{"value": "MJ"}], "type": "unit group data set", "refObjectId": "93a60a57-a3c8-11da-a746-0800200c9a66", "uri": "../unitgroups/93a60a57-a3c8-11da-a746-0800200c9a66"}}]}, "resolvedFlowVersion": "38.00.000", "flowProperties": [], "typeOfFlow": "Other flow", "classification": {"classHierarchy": "Quantities / Environmental quantities / EPD EN 15804 / LCI indicators", "name": "GaBiCategories"}}, {"dataSetInternalID": 4, "referenceToFlowDataSet": {"shortDescription": [{"value": "Exportierte thermische Energie (EET)", "lang": "de"}, {"value": "Exported thermal energy (EET)", "lang": "en"}, {"value": "Energía exportada termal (EET)", "lang": "es"}, {"value": "Exporterad energi – termisk (EET)", "lang": "sv"}], "type": "flow data set", "refObjectId": "98daf38a-7a79-46d3-9a37-2b7bd0955810", "version": "30.00.002"}, "exchange direction": "OUTPUT", "meanAmount": 0.0, "other": {"anies": [{"value": "0.0", "module": "A1", "scenario": "Standard scenario"}, {"value": "0.0", "module": "A2", "scenario": "Standard scenario"}, {"value": "-0.108710310440081", "module": "A3", "scenario": "Standard scenario"}, {"value": "0.0", "module": "A4", "scenario": "Standard scenario"}, {"value": "0.0", "module": "A5", "scenario": "Standard scenario"}, {"value": "0.0", "module": "B1", "scenario": "Standard scenario"}, {"value": "0.0", "module": "B2", "scenario": "Standard scenario"}, {"value": "0.0", "module": "B3", "scenario": "Standard scenario"}, {"value": "0.0", "module": "B4", "scenario": "Standard scenario"}, {"value": "0.0", "module": "B5", "scenario": "Standard scenario"}, {"value": "0.0", "module": "B6", "scenario": "Standard scenario"}, {"value": "0.0", "module": "B7", "scenario": "Standard scenario"}, {"value": "0.0", "module": "C1", "scenario": "Standard scenario"}, {"value": "0.0", "module": "C2", "scenario": "Standard scenario"}, {"value": "0.0", "module": "C3", "scenario": "Standard scenario"}, {"value": "0.0", "module": "C4", "scenario": "Standard scenario"}, {"value": "-0.247488269446359", "module": "D", "scenario": "Standard scenario"}, {"name": "referenceToUnitGroupDataSet", "value": {"shortDescription": [{"value": "MJ"}], "type": "unit group data set", "refObjectId": "93a60a57-a3c8-11da-a746-0800200c9a66", "uri": "../unitgroups/93a60a57-a3c8-11da-a746-0800200c9a66"}}]}, "resolvedFlowVersion": "38.00.000", "flowProperties": [], "typeOfFlow": "Other flow", "classification": {"classHierarchy": "Quantities / Environmental quantities / EPD EN 15804 / LCI indicators", "name": "GaBiCategories"}}, {"dataSetInternalID": 5, "referenceToFlowDataSet": {"shortDescription": [{"value": "Gefährlicher Abfall zur Deponie (HWD)", "lang": "de"}, {"value": "Hazardous waste disposed (HWD)", "lang": "en"}, {"value": "Residuos peligrosos eliminados (HWD)", "lang": "es"}, {"value": "Farligt avfall (HWD)", "lang": "sv"}], "type": "flow data set", "refObjectId": "430f9e0f-59b2-46a0-8e0d-55e0e84948fc", "version": "30.00.002"}, "exchange direction": "OUTPUT", "meanAmount": 0.0, "other": {"anies": [{"value": "5.91930182415E-5", "module": "A1", "scenario": "Standard scenario"}, {"value": "6.5799182174E-6", "module": "A2", "scenario": "Standard scenario"}, {"value": "5.57887688007E-5", "module": "A3", "scenario": "Standard scenario"}, {"value": "3.5573318791E-6", "module": "A4", "scenario": "Standard scenario"}, {"value": "5.83290753E-8", "module": "A5", "scenario": "Standard scenario"}, {"value": "0.0", "module": "B1", "scenario": "Standard scenario"}, {"value": "0.0", "module": "B2", "scenario": "Standard scenario"}, {"value": "0.0", "module": "B3", "scenario": "Standard scenario"}, {"value": "0.0", "module": "B4", "scenario": "Standard scenario"}, {"value": "0.0", "module": "B5", "scenario": "Standard scenario"}, {"value": "0.0", "module": "B6", "scenario": "Standard scenario"}, {"value": "0.0", "module": "B7", "scenario": "Standard scenario"}, {"value": "0.0", "module": "C1", "scenario": "Standard scenario"}, {"value": "2.767911864E-7", "module": "C2", "scenario": "Standard scenario"}, {"value": "9.98711235E-7", "module": "C3", "scenario": "Standard scenario"}, {"value": "1.50607885E-8", "module": "C4", "scenario": "Standard scenario"}, {"value": "-1.08053371369E-5", "module": "D", "scenario": "Standard scenario"}, {"name": "referenceToUnitGroupDataSet", "value": {"shortDescription": [{"value": "kg"}], "type": "unit group data set", "refObjectId": "ad38d542-3fe9-439d-9b95-2f5f7752acaf", "uri": "../unitgroups/ad38d542-3fe9-439d-9b95-2f5f7752acaf"}}]}, "resolvedFlowVersion": "38.00.000", "flowProperties": [], "typeOfFlow": "Other flow", "classification": {"classHierarchy": "Quantities / Environmental quantities / EPD EN 15804 / LCI indicators", "name": "GaBiCategories"}}, {"dataSetInternalID": 6, "referenceToFlowDataSet": {"shortDescription": [{"value": "Stoffe für die Energierückgewinnung (MER)", "lang": "de"}, {"value": "Materials for energy recovery (MER)", "lang": "en"}, {"value": "Materiales para valorización energética (recuperación de energía) (MER)", "lang": "es"}, {"value": "Material till energiåtervinning (MER)", "lang": "sv"}], "type": "flow data set", "refObjectId": "59a9181c-3aaf-46ee-8b13-2b3723b6e447", "version": "30.00.002"}, "exchange direction": "OUTPUT", "meanAmount": 0.0, "other": {"anies": [{"value": "0.0", "module": "A1", "scenario": "Standard scenario"}, {"value": "0.0", "module": "A2", "scenario": "Standard scenario"}, {"value": "0.0", "module": "A3", "scenario": "Standard scenario"}, {"value": "0.0", "module": "A4", "scenario": "Standard scenario"}, {"value": "0.0", "module": "A5", "scenario": "Standard scenario"}, {"value": "0.0", "module": "B1", "scenario": "Standard scenario"}, {"value": "0.0", "module": "B2", "scenario": "Standard scenario"}, {"value": "0.0", "module": "B3", "scenario": "Standard scenario"}, {"value": "0.0", "module": "B4", "scenario": "Standard scenario"}, {"value": "0.0", "module": "B5", "scenario": "Standard scenario"}, {"value": "0.0", "module": "B6", "scenario": "Standard scenario"}, {"value": "0.0", "module": "B7", "scenario": "Standard scenario"}, {"value": "0.0", "module": "C1", "scenario": "Standard scenario"}, {"value": "0.0", "module": "C2", "scenario": "Standard scenario"}, {"value": "0.0", "module": "C3", "scenario": "Standard scenario"}, {"value": "0.0", "module": "C4", "scenario": "Standard scenario"}, {"value": "0.0", "module": "D", "scenario": "Standard scenario"}, {"name": "referenceToUnitGroupDataSet", "value": {"shortDescription": [{"value": "kg"}], "type": "unit group data set", "refObjectId": "ad38d542-3fe9-439d-9b95-2f5f7752acaf", "uri": "../unitgroups/ad38d542-3fe9-439d-9b95-2f5f7752acaf"}}]}, "resolvedFlowVersion": "38.00.000", "flowProperties": [], "typeOfFlow": "Other flow", "classification": {"classHierarchy": "Quantities / Environmental quantities / EPD EN 15804 / LCI indicators", "name": "GaBiCategories"}}, {"dataSetInternalID": 7, "referenceToFlowDataSet": {"shortDescription": [{"value": "Stoffe zum Recycling (MFR)", "lang": "de"}, {"value": "Materials for recycling (MFR)", "lang": "en"}, {"value": "Materiales para el reciclaje (MFR)", "lang": "es"}, {"value": "Material till återvinning (MFR)", "lang": "sv"}], "type": "flow data set", "refObjectId": "d7fe48a5-4103-49c8-9aae-b0b5dfdbd6ae", "version": "30.00.002"}, "exchange direction": "OUTPUT", "meanAmount": 0.0, "other": {"anies": [{"value": "0.0", "module": "A1", "scenario": "Standard scenario"}, {"value": "0.0", "module": "A2", "scenario": "Standard scenario"}, {"value": "0.16872399", "module": "A3", "scenario": "Standard scenario"}, {"value": "0.0", "module": "A4", "scenario": "Standard scenario"}, {"value": "0.005861249499", "module": "A5", "scenario": "Standard scenario"}, {"value": "0.0", "module": "B1", "scenario": "Standard scenario"}, {"value": "0.0", "module": "B2", "scenario": "Standard scenario"}, {"value": "0.0", "module": "B3", "scenario": "Standard scenario"}, {"value": "0.0", "module": "B4", "scenario": "Standard scenario"}, {"value": "0.0", "module": "B5", "scenario": "Standard scenario"}, {"value": "0.0", "module": "B6", "scenario": "Standard scenario"}, {"value": "0.0", "module": "B7", "scenario": "Standard scenario"}, {"value": "0.0", "module": "C1", "scenario": "Standard scenario"}, {"value": "0.0", "module": "C2", "scenario": "Standard scenario"}, {"value": "0.938020999999999", "module": "C3", "scenario": "Standard scenario"}, {"value": "0.0", "module": "C4", "scenario": "Standard scenario"}, {"value": "0.0", "module": "D", "scenario": "Standard scenario"}, {"name": "referenceToUnitGroupDataSet", "value": {"shortDescription": [{"value": "kg"}], "type": "unit group data set", "refObjectId": "ad38d542-3fe9-439d-9b95-2f5f7752acaf", "uri": "../unitgroups/ad38d542-3fe9-439d-9b95-2f5f7752acaf"}}]}, "resolvedFlowVersion": "38.00.000", "flowProperties": [], "typeOfFlow": "Other flow", "classification": {"classHierarchy": "Quantities / Environmental quantities / EPD EN 15804 / LCI indicators", "name": "GaBiCategories"}}, {"dataSetInternalID": 8, "referenceToFlowDataSet": {"shortDescription": [{"value": "Einsatz von Süßwasserressourcen (FW)", "lang": "de"}, {"value": "Use of net fresh water (FW)", "lang": "en"}, {"value": "Uso neto de recursos de agua dulce (FW)", "lang": "es"}, {"value": "Användning av sötvatten (FW)", "lang": "sv"}], "type": "flow data set", "refObjectId": "3cf952c8-f3a4-461d-8c96-96456ca62246", "version": "30.00.003"}, "exchange direction": "INPUT", "meanAmount": 0.0, "other": {"anies": [{"value": "0.0369482994380689", "module": "A1", "scenario": "Standard scenario"}, {"value": "3.088729425039E-4", "module": "A2", "scenario": "Standard scenario"}, {"value": "0.005649661969255", "module": "A3", "scenario": "Standard scenario"}, {"value": "1.709983021879E-4", "module": "A4", "scenario": "Standard scenario"}, {"value": "2.75917631564E-5", "module": "A5", "scenario": "Standard scenario"}, {"value": "0.0", "module": "B1", "scenario": "Standard scenario"}, {"value": "0.0", "module": "B2", "scenario": "Standard scenario"}, {"value": "0.0", "module": "B3", "scenario": "Standard scenario"}, {"value": "0.0", "module": "B4", "scenario": "Standard scenario"}, {"value": "0.0", "module": "B5", "scenario": "Standard scenario"}, {"value": "0.0", "module": "B6", "scenario": "Standard scenario"}, {"value": "0.0", "module": "B7", "scenario": "Standard scenario"}, {"value": "0.0", "module": "C1", "scenario": "Standard scenario"}, {"value": "1.33051468212E-5", "module": "C2", "scenario": "Standard scenario"}, {"value": "1.991586585E-4", "module": "C3", "scenario": "Standard scenario"}, {"value": "1.5149072E-5", "module": "C4", "scenario": "Standard scenario"}, {"value": "-0.014446225374245", "module": "D", "scenario": "Standard scenario"}, {"name": "referenceToUnitGroupDataSet", "value": {"shortDescription": [{"value": "m3"}], "type": "unit group data set", "refObjectId": "cd950537-0a98-4044-9ba7-9f9a68d0a504", "uri": "../unitgroups/cd950537-0a98-4044-9ba7-9f9a68d0a504"}}]}, "resolvedFlowVersion": "38.00.000", "flowProperties": [], "typeOfFlow": "Other flow", "classification": {"classHierarchy": "Quantities / Environmental quantities / EPD EN 15804 / LCI indicators", "name": "GaBiCategories"}}, {"dataSetInternalID": 9, "referenceToFlowDataSet": {"shortDescription": [{"value": "Entsorgter nicht gefährlicher Abfall (NHWD)", "lang": "de"}, {"value": "Non hazardous waste dispose (NHWD)", "lang": "en"}, {"value": "Residuos no peligrosos eliminados (NHWD)", "lang": "es"}, {"value": "Icke-farligt avfall (NHWD)", "lang": "sv"}], "type": "flow data set", "refObjectId": "b29ef66b-e286-4afa-949f-62f1a7b4d7fa", "version": "30.00.002"}, "exchange direction": "OUTPUT", "meanAmount": 0.0, "other": {"anies": [{"value": "0.692751892166025", "module": "A1", "scenario": "Standard scenario"}, {"value": "0.158074869340257", "module": "A2", "scenario": "Standard scenario"}, {"value": "0.162021688992457", "module": "A3", "scenario": "Standard scenario"}, {"value": "0.0890471255050057", "module": "A4", "scenario": "Standard scenario"}, {"value": "0.0033680545905747", "module": "A5", "scenario": "Standard scenario"}, {"value": "0.0", "module": "B1", "scenario": "Standard scenario"}, {"value": "0.0", "module": "B2", "scenario": "Standard scenario"}, {"value": "0.0", "module": "B3", "scenario": "Standard scenario"}, {"value": "0.0", "module": "B4", "scenario": "Standard scenario"}, {"value": "0.0", "module": "B5", "scenario": "Standard scenario"}, {"value": "0.0", "module": "B6", "scenario": "Standard scenario"}, {"value": "0.0", "module": "B7", "scenario": "Standard scenario"}, {"value": "0.0", "module": "C1", "scenario": "Standard scenario"}, {"value": "0.0069286365050806", "module": "C2", "scenario": "Standard scenario"}, {"value": "0.0103231815785", "module": "C3", "scenario": "Standard scenario"}, {"value": "0.0507729608255", "module": "C4", "scenario": "Standard scenario"}, {"value": "-0.508886950750364", "module": "D", "scenario": "Standard scenario"}, {"name": "referenceToUnitGroupDataSet", "value": {"shortDescription": [{"value": "kg"}], "type": "unit group data set", "refObjectId": "ad38d542-3fe9-439d-9b95-2f5f7752acaf", "uri": "../unitgroups/ad38d542-3fe9-439d-9b95-2f5f7752acaf"}}]}, "resolvedFlowVersion": "38.00.000", "flowProperties": [], "typeOfFlow": "Other flow", "classification": {"classHierarchy": "Quantities / Environmental quantities / EPD EN 15804 / LCI indicators", "name": "GaBiCategories"}}, {"dataSetInternalID": 10, "referenceToFlowDataSet": {"shortDescription": [{"value": "Nicht-erneuerbare Primärenergie als Energieträger (PENRE)", "lang": "de"}, {"value": "Use of non renewable primary energy (PENRE)", "lang": "en"}, {"value": "Uso de energía primaria no renovable, excluyendo los recursos de energía primaria no renovable utilizada como materia prima (PENRE)", "lang": "es"}, {"value": "Icke förnybar primärenergi - använd som energibärare (PENRE)", "lang": "sv"}], "type": "flow data set", "refObjectId": "ac857178-2b45-46ec-892a-a9a4332f0372", "version": "30.00.002"}, "exchange direction": "INPUT", "meanAmount": 0.0, "other": {"anies": [{"value": "27.5494369586676", "module": "A1", "scenario": "Standard scenario"}, {"value": "2.74284652277569", "module": "A2", "scenario": "Standard scenario"}, {"value": "6.46550617003989", "module": "A3", "scenario": "Standard scenario"}, {"value": "1.49044518897716", "module": "A4", "scenario": "Standard scenario"}, {"value": "0.0241531110704826", "module": "A5", "scenario": "Standard scenario"}, {"value": "0.0", "module": "B1", "scenario": "Standard scenario"}, {"value": "0.0", "module": "B2", "scenario": "Standard scenario"}, {"value": "0.0", "module": "B3", "scenario": "Standard scenario"}, {"value": "0.0", "module": "B4", "scenario": "Standard scenario"}, {"value": "0.0", "module": "B5", "scenario": "Standard scenario"}, {"value": "0.0", "module": "B6", "scenario": "Standard scenario"}, {"value": "0.0", "module": "B7", "scenario": "Standard scenario"}, {"value": "0.0", "module": "C1", "scenario": "Standard scenario"}, {"value": "0.115969526097598", "module": "C2", "scenario": "Standard scenario"}, {"value": "0.3477478495155", "module": "C3", "scenario": "Standard scenario"}, {"value": "0.0129317028885", "module": "C4", "scenario": "Standard scenario"}, {"value": "-9.20752168748779", "module": "D", "scenario": "Standard scenario"}, {"name": "referenceToUnitGroupDataSet", "value": {"shortDescription": [{"value": "MJ"}], "type": "unit group data set", "refObjectId": "93a60a57-a3c8-11da-a746-0800200c9a66", "uri": "../unitgroups/93a60a57-a3c8-11da-a746-0800200c9a66"}}]}, "resolvedFlowVersion": "38.00.000", "flowProperties": [], "typeOfFlow": "Other flow", "classification": {"classHierarchy": "Quantities", "name": "GaBiCategories"}}, {"dataSetInternalID": 11, "referenceToFlowDataSet": {"shortDescription": [{"value": "Nicht-erneuerbare Primärenergie zur stofflichen Nutzung (PENRM)", "lang": "de"}, {"value": "Use of non renewable primary energy resources used as raw materials (PENRM)", "lang": "en"}, {"value": "Uso de la energía primaria no renovable utilizada como materia prima (PENRM)", "lang": "es"}, {"value": "Icke förnybar primärenergi - använd som råmaterial (PENRM)", "lang": "sv"}], "type": "flow data set", "refObjectId": "1421caa0-679d-4bf4-b282-0eb850ccae27", "version": "30.00.001"}, "exchange direction": "INPUT", "meanAmount": 0.0, "other": {"anies": [{"value": "0.3618989", "module": "A1", "scenario": "Standard scenario"}, {"value": "0.0", "module": "A2", "scenario": "Standard scenario"}, {"value": "0.393148420774454", "module": "A3", "scenario": "Standard scenario"}, {"value": "0.0", "module": "A4", "scenario": "Standard scenario"}, {"value": "7.55047320774E-5", "module": "A5", "scenario": "Standard scenario"}, {"value": "0.0", "module": "B1", "scenario": "Standard scenario"}, {"value": "0.0", "module": "B2", "scenario": "Standard scenario"}, {"value": "0.0", "module": "B3", "scenario": "Standard scenario"}, {"value": "0.0", "module": "B4", "scenario": "Standard scenario"}, {"value": "0.0", "module": "B5", "scenario": "Standard scenario"}, {"value": "0.0", "module": "B6", "scenario": "Standard scenario"}, {"value": "0.0", "module": "B7", "scenario": "Standard scenario"}, {"value": "0.0", "module": "C1", "scenario": "Standard scenario"}, {"value": "0.0", "module": "C2", "scenario": "Standard scenario"}, {"value": "0.0", "module": "C3", "scenario": "Standard scenario"}, {"value": "0.0", "module": "C4", "scenario": "Standard scenario"}, {"value": "-0.020361516898095", "module": "D", "scenario": "Standard scenario"}, {"name": "referenceToUnitGroupDataSet", "value": {"shortDescription": [{"value": "MJ"}], "type": "unit group data set", "refObjectId": "93a60a57-a3c8-11da-a746-0800200c9a66", "uri": "../unitgroups/93a60a57-a3c8-11da-a746-0800200c9a66"}}]}, "resolvedFlowVersion": "38.00.000", "flowProperties": [], "typeOfFlow": "Other flow", "classification": {"classHierarchy": "Quantities", "name": "GaBiCategories"}}, {"dataSetInternalID": 12, "referenceToFlowDataSet": {"shortDescription": [{"value": "Nicht erneuerbare Sekundärbrennstoffe (NRSF)", "lang": "de"}, {"value": "Use of non renewable secondary fuels (NRSF)", "lang": "en"}, {"value": "Uso de combustibles secundarios no renovables (NRSF)", "lang": "es"}, {"value": "Användning av ickeförnybara sekundära bränslen (NRSF)", "lang": "sv"}], "type": "flow data set", "refObjectId": "89def144-d39a-4287-b86f-efde453ddcb2", "version": "30.00.001"}, "exchange direction": "INPUT", "meanAmount": 0.0, "other": {"anies": [{"value": "0.0", "module": "A1", "scenario": "Standard scenario"}, {"value": "0.0", "module": "A2", "scenario": "Standard scenario"}, {"value": "0.0", "module": "A3", "scenario": "Standard scenario"}, {"value": "0.0", "module": "A4", "scenario": "Standard scenario"}, {"value": "0.0", "module": "A5", "scenario": "Standard scenario"}, {"value": "0.0", "module": "B1", "scenario": "Standard scenario"}, {"value": "0.0", "module": "B2", "scenario": "Standard scenario"}, {"value": "0.0", "module": "B3", "scenario": "Standard scenario"}, {"value": "0.0", "module": "B4", "scenario": "Standard scenario"}, {"value": "0.0", "module": "B5", "scenario": "Standard scenario"}, {"value": "0.0", "module": "B6", "scenario": "Standard scenario"}, {"value": "0.0", "module": "B7", "scenario": "Standard scenario"}, {"value": "0.0", "module": "C1", "scenario": "Standard scenario"}, {"value": "0.0", "module": "C2", "scenario": "Standard scenario"}, {"value": "0.0", "module": "C3", "scenario": "Standard scenario"}, {"value": "0.0", "module": "C4", "scenario": "Standard scenario"}, {"value": "0.0", "module": "D", "scenario": "Standard scenario"}, {"name": "referenceToUnitGroupDataSet", "value": {"shortDescription": [{"value": "MJ"}], "type": "unit group data set", "refObjectId": "93a60a57-a3c8-11da-a746-0800200c9a66", "uri": "../unitgroups/93a60a57-a3c8-11da-a746-0800200c9a66"}}]}, "resolvedFlowVersion": "38.00.000", "flowProperties": [], "typeOfFlow": "Other flow", "classification": {"classHierarchy": "Quantities / Environmental quantities / EPD EN 15804 / LCI indicators", "name": "GaBiCategories"}}, {"dataSetInternalID": 13, "referenceToFlowDataSet": {"shortDescription": [{"value": "Entsorgter radioaktiver Abfall (RWD)", "lang": "de"}, {"value": "Radioactive waste disposed (RWD)", "lang": "en"}, {"value": "Residuos radiactivos eliminados (RWD)", "lang": "es"}, {"value": "Radioaktivt avfall (RWD) ", "lang": "sv"}], "type": "flow data set", "refObjectId": "3449546e-52ad-4b39-b809-9fb77cea8ff6", "version": "30.00.001"}, "exchange direction": "OUTPUT", "meanAmount": 0.0, "other": {"anies": [{"value": "1.076817742802E-4", "module": "A1", "scenario": "Standard scenario"}, {"value": "1.70603349548E-5", "module": "A2", "scenario": "Standard scenario"}, {"value": "3.10963298605E-5", "module": "A3", "scenario": "Standard scenario"}, {"value": "9.2181633224E-6", "module": "A4", "scenario": "Standard scenario"}, {"value": "1.250703551E-7", "module": "A5", "scenario": "Standard scenario"}, {"value": "0.0", "module": "B1", "scenario": "Standard scenario"}, {"value": "0.0", "module": "B2", "scenario": "Standard scenario"}, {"value": "0.0", "module": "B3", "scenario": "Standard scenario"}, {"value": "0.0", "module": "B4", "scenario": "Standard scenario"}, {"value": "0.0", "module": "B5", "scenario": "Standard scenario"}, {"value": "0.0", "module": "B6", "scenario": "Standard scenario"}, {"value": "0.0", "module": "B7", "scenario": "Standard scenario"}, {"value": "0.0", "module": "C1", "scenario": "Standard scenario"}, {"value": "7.172528315E-7", "module": "C2", "scenario": "Standard scenario"}, {"value": "1.92848669E-6", "module": "C3", "scenario": "Standard scenario"}, {"value": "8.0425045E-8", "module": "C4", "scenario": "Standard scenario"}, {"value": "-3.72334107032E-5", "module": "D", "scenario": "Standard scenario"}, {"name": "referenceToUnitGroupDataSet", "value": {"shortDescription": [{"value": "kg"}], "type": "unit group data set", "refObjectId": "ad38d542-3fe9-439d-9b95-2f5f7752acaf", "uri": "../unitgroups/ad38d542-3fe9-439d-9b95-2f5f7752acaf"}}]}, "resolvedFlowVersion": "38.00.000", "flowProperties": [], "typeOfFlow": "Other flow", "classification": {"classHierarchy": "Quantities / Environmental quantities / EPD EN 15804 / LCI indicators", "name": "GaBiCategories"}}, {"dataSetInternalID": 14, "referenceToFlowDataSet": {"shortDescription": [{"value": "Erneuerbare Primärenergie als Energieträger (PERE)", "lang": "de"}, {"value": "Use of renewable primary energy (PERE)", "lang": "en"}, {"value": "Uso de energía primaria renovable excluyendo los recursos de energía primaria renovable utilizada como materia prima (PERE)", "lang": "es"}, {"value": "Förnybar energi - använd som energibärare (PERE)", "lang": "sv"}], "type": "flow data set", "refObjectId": "20f32be5-0398-4288-9b6d-accddd195317", "version": "30.00.001"}, "exchange direction": "INPUT", "meanAmount": 0.0, "other": {"anies": [{"value": "6.15142262813613", "module": "A1", "scenario": "Standard scenario"}, {"value": "0.0330460161676971", "module": "A2", "scenario": "Standard scenario"}, {"value": "5.01101908380863", "module": "A3", "scenario": "Standard scenario"}, {"value": "0.0175745372519186", "module": "A4", "scenario": "Standard scenario"}, {"value": "0.0018237428690407", "module": "A5", "scenario": "Standard scenario"}, {"value": "0.0", "module": "B1", "scenario": "Standard scenario"}, {"value": "0.0", "module": "B2", "scenario": "Standard scenario"}, {"value": "0.0", "module": "B3", "scenario": "Standard scenario"}, {"value": "0.0", "module": "B4", "scenario": "Standard scenario"}, {"value": "0.0", "module": "B5", "scenario": "Standard scenario"}, {"value": "0.0", "module": "B6", "scenario": "Standard scenario"}, {"value": "0.0", "module": "B7", "scenario": "Standard scenario"}, {"value": "0.0", "module": "C1", "scenario": "Standard scenario"}, {"value": "0.0013674509948858", "module": "C2", "scenario": "Standard scenario"}, {"value": "0.050661967943", "module": "C3", "scenario": "Standard scenario"}, {"value": "6.741481045E-4", "module": "C4", "scenario": "Standard scenario"}, {"value": "-3.3476040218966", "module": "D", "scenario": "Standard scenario"}, {"name": "referenceToUnitGroupDataSet", "value": {"shortDescription": [{"value": "MJ"}], "type": "unit group data set", "refObjectId": "93a60a57-a3c8-11da-a746-0800200c9a66", "uri": "../unitgroups/93a60a57-a3c8-11da-a746-0800200c9a66"}}]}, "resolvedFlowVersion": "38.00.000", "flowProperties": [], "typeOfFlow": "Other flow", "classification": {"classHierarchy": "Quantities", "name": "GaBiCategories"}}, {"dataSetInternalID": 15, "referenceToFlowDataSet": {"shortDescription": [{"value": "Erneuerbare Primärenergie zur stofflichen Nutzung (PERM)", "lang": "de"}, {"value": "Use of renewable primary energy resources used as raw materials (PERM)", "lang": "en"}, {"value": "Uso de energía primaria renovable utilizada como materia prima (PERM)", "lang": "es"}, {"value": "Förnybar energi - använd som råmaterial (PERM)", "lang": "sv"}], "type": "flow data set", "refObjectId": "fb3ec0de-548d-4508-aea5-00b73bf6f702", "version": "30.00.001"}, "exchange direction": "INPUT", "meanAmount": 0.0, "other": {"anies": [{"value": "0.0", "module": "A1", "scenario": "Standard scenario"}, {"value": "0.0", "module": "A2", "scenario": "Standard scenario"}, {"value": "0.590041", "module": "A3", "scenario": "Standard scenario"}, {"value": "0.0", "module": "A4", "scenario": "Standard scenario"}, {"value": "5.90041E-5", "module": "A5", "scenario": "Standard scenario"}, {"value": "0.0", "module": "B1", "scenario": "Standard scenario"}, {"value": "0.0", "module": "B2", "scenario": "Standard scenario"}, {"value": "0.0", "module": "B3", "scenario": "Standard scenario"}, {"value": "0.0", "module": "B4", "scenario": "Standard scenario"}, {"value": "0.0", "module": "B5", "scenario": "Standard scenario"}, {"value": "0.0", "module": "B6", "scenario": "Standard scenario"}, {"value": "0.0", "module": "B7", "scenario": "Standard scenario"}, {"value": "0.0", "module": "C1", "scenario": "Standard scenario"}, {"value": "0.0", "module": "C2", "scenario": "Standard scenario"}, {"value": "0.0", "module": "C3", "scenario": "Standard scenario"}, {"value": "0.0", "module": "C4", "scenario": "Standard scenario"}, {"value": "0.0", "module": "D", "scenario": "Standard scenario"}, {"name": "referenceToUnitGroupDataSet", "value": {"shortDescription": [{"value": "MJ"}], "type": "unit group data set", "refObjectId": "93a60a57-a3c8-11da-a746-0800200c9a66", "uri": "../unitgroups/93a60a57-a3c8-11da-a746-0800200c9a66"}}]}, "resolvedFlowVersion": "38.00.000", "flowProperties": [], "typeOfFlow": "Other flow", "classification": {"classHierarchy": "Quantities", "name": "GaBiCategories"}}, {"dataSetInternalID": 16, "referenceToFlowDataSet": {"shortDescription": [{"value": "Erneuerbare Sekundärbrennstoffe (RSF)", "lang": "de"}, {"value": "Use of renewable secondary fuels (RSF)", "lang": "en"}, {"value": "Uso de combustibles secundarios renovables (RSF)", "lang": "es"}, {"value": "Användning av förnybara sekundära bränslen (RSF)", "lang": "sv"}], "type": "flow data set", "refObjectId": "64333088-a55f-4aa2-9a31-c10b07816787", "version": "30.00.001"}, "exchange direction": "INPUT", "meanAmount": 0.0, "other": {"anies": [{"value": "0.0", "module": "A1", "scenario": "Standard scenario"}, {"value": "0.0", "module": "A2", "scenario": "Standard scenario"}, {"value": "0.0", "module": "A3", "scenario": "Standard scenario"}, {"value": "0.0", "module": "A4", "scenario": "Standard scenario"}, {"value": "0.0", "module": "A5", "scenario": "Standard scenario"}, {"value": "0.0", "module": "B1", "scenario": "Standard scenario"}, {"value": "0.0", "module": "B2", "scenario": "Standard scenario"}, {"value": "0.0", "module": "B3", "scenario": "Standard scenario"}, {"value": "0.0", "module": "B4", "scenario": "Standard scenario"}, {"value": "0.0", "module": "B5", "scenario": "Standard scenario"}, {"value": "0.0", "module": "B6", "scenario": "Standard scenario"}, {"value": "0.0", "module": "B7", "scenario": "Standard scenario"}, {"value": "0.0", "module": "C1", "scenario": "Standard scenario"}, {"value": "0.0", "module": "C2", "scenario": "Standard scenario"}, {"value": "0.0", "module": "C3", "scenario": "Standard scenario"}, {"value": "0.0", "module": "C4", "scenario": "Standard scenario"}, {"value": "0.0", "module": "D", "scenario": "Standard scenario"}, {"name": "referenceToUnitGroupDataSet", "value": {"shortDescription": [{"value": "MJ"}], "type": "unit group data set", "refObjectId": "93a60a57-a3c8-11da-a746-0800200c9a66", "uri": "../unitgroups/93a60a57-a3c8-11da-a746-0800200c9a66"}}]}, "resolvedFlowVersion": "38.00.000", "flowProperties": [], "typeOfFlow": "Other flow", "classification": {"classHierarchy": "Quantities / Environmental quantities / EPD EN 15804 / LCI indicators", "name": "GaBiCategories"}}, {"dataSetInternalID": 17, "referenceToFlowDataSet": {"shortDescription": [{"value": "Einsatz von Sekundärstoffen (SM)", "lang": "de"}, {"value": "Use of secondary material (SM)", "lang": "en"}, {"value": "Uso de materiales secundarios (SM)", "lang": "es"}, {"value": "Användning av sekundära material (SM)", "lang": "sv"}], "type": "flow data set", "refObjectId": "c6a1f35f-2d09-4f54-8dfb-97e502e1ce92", "version": "30.00.001"}, "exchange direction": "INPUT", "meanAmount": 0.0, "other": {"anies": [{"value": "0.54722419414", "module": "A1", "scenario": "Standard scenario"}, {"value": "0.0", "module": "A2", "scenario": "Standard scenario"}, {"value": "0.0985003549452", "module": "A3", "scenario": "Standard scenario"}, {"value": "0.0", "module": "A4", "scenario": "Standard scenario"}, {"value": "6.45724549085E-5", "module": "A5", "scenario": "Standard scenario"}, {"value": "0.0", "module": "B1", "scenario": "Standard scenario"}, {"value": "0.0", "module": "B2", "scenario": "Standard scenario"}, {"value": "0.0", "module": "B3", "scenario": "Standard scenario"}, {"value": "0.0", "module": "B4", "scenario": "Standard scenario"}, {"value": "0.0", "module": "B5", "scenario": "Standard scenario"}, {"value": "0.0", "module": "B6", "scenario": "Standard scenario"}, {"value": "0.0", "module": "B7", "scenario": "Standard scenario"}, {"value": "0.0", "module": "C1", "scenario": "Standard scenario"}, {"value": "0.0", "module": "C2", "scenario": "Standard scenario"}, {"value": "0.0", "module": "C3", "scenario": "Standard scenario"}, {"value": "0.0", "module": "C4", "scenario": "Standard scenario"}, {"value": "0.0", "module": "D", "scenario": "Standard scenario"}, {"name": "referenceToUnitGroupDataSet", "value": {"shortDescription": [{"value": "kg"}], "type": "unit group data set", "refObjectId": "ad38d542-3fe9-439d-9b95-2f5f7752acaf", "uri": "../unitgroups/ad38d542-3fe9-439d-9b95-2f5f7752acaf"}}]}, "resolvedFlowVersion": "38.00.000", "flowProperties": [], "typeOfFlow": "Other flow", "classification": {"classHierarchy": "Quantities / Environmental quantities / EPD EN 15804 / LCI indicators", "name": "GaBiCategories"}}, {"dataSetInternalID": 18, "referenceToFlowDataSet": {"shortDescription": [{"value": "Total nicht erneuerbare Primärenergie (PENRT)", "lang": "de"}, {"value": "Total use of non renewable primary energy resource (PENRT)", "lang": "en"}, {"value": "Uso total de la energía primaria no renovable (energía primaria y recursos de energía primaria renovable utilizada como materia prima) (PENRT)", "lang": "es"}, {"value": "Icke förnybar primärenergi – total (PENRT)", "lang": "sv"}], "type": "flow data set", "refObjectId": "06159210-646b-4c8d-8583-da9b3b95a6c1", "version": "30.00.001"}, "exchange direction": "INPUT", "meanAmount": 0.0, "other": {"anies": [{"value": "27.9113358586676", "module": "A1", "scenario": "Standard scenario"}, {"value": "2.74284652277569", "module": "A2", "scenario": "Standard scenario"}, {"value": "6.85865459081434", "module": "A3", "scenario": "Standard scenario"}, {"value": "1.49044518897716", "module": "A4", "scenario": "Standard scenario"}, {"value": "0.0242286158025601", "module": "A5", "scenario": "Standard scenario"}, {"value": "0.0", "module": "B1", "scenario": "Standard scenario"}, {"value": "0.0", "module": "B2", "scenario": "Standard scenario"}, {"value": "0.0", "module": "B3", "scenario": "Standard scenario"}, {"value": "0.0", "module": "B4", "scenario": "Standard scenario"}, {"value": "0.0", "module": "B5", "scenario": "Standard scenario"}, {"value": "0.0", "module": "B6", "scenario": "Standard scenario"}, {"value": "0.0", "module": "B7", "scenario": "Standard scenario"}, {"value": "0.0", "module": "C1", "scenario": "Standard scenario"}, {"value": "0.115969526097598", "module": "C2", "scenario": "Standard scenario"}, {"value": "0.3477478495155", "module": "C3", "scenario": "Standard scenario"}, {"value": "0.0129317028885", "module": "C4", "scenario": "Standard scenario"}, {"value": "-9.22788320438589", "module": "D", "scenario": "Standard scenario"}, {"name": "referenceToUnitGroupDataSet", "value": {"shortDescription": [{"value": "MJ"}], "type": "unit group data set", "refObjectId": "93a60a57-a3c8-11da-a746-0800200c9a66", "uri": "../unitgroups/93a60a57-a3c8-11da-a746-0800200c9a66"}}]}, "resolvedFlowVersion": "38.00.000", "flowProperties": [], "typeOfFlow": "Other flow", "classification": {"classHierarchy": "Quantities / Environmental quantities / EPD EN 15804 / LCI indicators", "name": "GaBiCategories"}}, {"dataSetInternalID": 19, "referenceToFlowDataSet": {"shortDescription": [{"value": "Total erneuerbare Primärenergie (PERT)", "lang": "de"}, {"value": "Total use of renewable primary energy resources (PERT)", "lang": "en"}, {"value": "Uso total de la energía primaria renovable (energía primaria y recursos de energía primaria renovable utilizada como materia prima) (PERT)", "lang": "es"}, {"value": "Förnybar energi – total (PERT)", "lang": "sv"}], "type": "flow data set", "refObjectId": "53f97275-fa8a-4cdd-9024-65936002acd0", "version": "30.00.001"}, "exchange direction": "INPUT", "meanAmount": 0.0, "other": {"anies": [{"value": "6.15142262813613", "module": "A1", "scenario": "Standard scenario"}, {"value": "0.0330460161676971", "module": "A2", "scenario": "Standard scenario"}, {"value": "5.60106008380863", "module": "A3", "scenario": "Standard scenario"}, {"value": "0.0175745372519186", "module": "A4", "scenario": "Standard scenario"}, {"value": "0.0018827469690407", "module": "A5", "scenario": "Standard scenario"}, {"value": "0.0", "module": "B1", "scenario": "Standard scenario"}, {"value": "0.0", "module": "B2", "scenario": "Standard scenario"}, {"value": "0.0", "module": "B3", "scenario": "Standard scenario"}, {"value": "0.0", "module": "B4", "scenario": "Standard scenario"}, {"value": "0.0", "module": "B5", "scenario": "Standard scenario"}, {"value": "0.0", "module": "B6", "scenario": "Standard scenario"}, {"value": "0.0", "module": "B7", "scenario": "Standard scenario"}, {"value": "0.0", "module": "C1", "scenario": "Standard scenario"}, {"value": "0.0013674509948858", "module": "C2", "scenario": "Standard scenario"}, {"value": "0.050661967943", "module": "C3", "scenario": "Standard scenario"}, {"value": "6.741481045E-4", "module": "C4", "scenario": "Standard scenario"}, {"value": "-3.3476040218966", "module": "D", "scenario": "Standard scenario"}, {"name": "referenceToUnitGroupDataSet", "value": {"shortDescription": [{"value": "MJ"}], "type": "unit group data set", "refObjectId": "93a60a57-a3c8-11da-a746-0800200c9a66", "uri": "../unitgroups/93a60a57-a3c8-11da-a746-0800200c9a66"}}]}, "resolvedFlowVersion": "38.00.000", "flowProperties": [], "typeOfFlow": "Other flow", "classification": {"classHierarchy": "Quantities / Environmental quantities / EPD EN 15804 / LCI indicators", "name": "GaBiCategories"}}]}, "LCIAResults": {"LCIAResult": [{"referenceToLCIAMethodDataSet": {"shortDescription": [{"value": "Potenzial für die Verknappung abiotischer Ressourcen – nicht fossile Ressourcen (ADPE)", "lang": "de"}, {"value": "Abiotic depletion potential - non-fossil resources (ADPE)", "lang": "en"}, {"value": "Abiotisk utarmningspotential icke fossila resurser (ADP-mm)", "lang": "sv"}], "type": "LCIA method data set", "refObjectId": "b2ad6494-c78d-11e6-9d9d-cec0c932ce01", "version": "01.00.012"}, "meanAmount": 0.0, "other": {"anies": [{"value": "7.893461562324E-4", "module": "A1", "scenario": "Standard scenario"}, {"value": "4.3970546959E-6", "module": "A2", "scenario": "Standard scenario"}, {"value": "6.64635041054E-5", "module": "A3", "scenario": "Standard scenario"}, {"value": "2.358305453E-6", "module": "A4", "scenario": "Standard scenario"}, {"value": "1.224968266E-7", "module": "A5", "scenario": "Standard scenario"}, {"value": "0.0", "module": "B1", "scenario": "Standard scenario"}, {"value": "0.0", "module": "B2", "scenario": "Standard scenario"}, {"value": "0.0", "module": "B3", "scenario": "Standard scenario"}, {"value": "0.0", "module": "B4", "scenario": "Standard scenario"}, {"value": "0.0", "module": "B5", "scenario": "Standard scenario"}, {"value": "0.0", "module": "B6", "scenario": "Standard scenario"}, {"value": "0.0", "module": "B7", "scenario": "Standard scenario"}, {"value": "0.0", "module": "C1", "scenario": "Standard scenario"}, {"value": "1.834965605E-7", "module": "C2", "scenario": "Standard scenario"}, {"value": "1.292583631E-6", "module": "C3", "scenario": "Standard scenario"}, {"value": "4.0379616E-9", "module": "C4", "scenario": "Standard scenario"}, {"value": "-4.759332616485E-4", "module": "D", "scenario": "Standard scenario"}, {"name": "referenceToUnitGroupDataSet", "value": {"shortDescription": [{"value": "kg Sb-Äqv."}], "type": "unit group data set", "refObjectId": "54ccd2d9-a32a-4fc2-923d-f2c8c93e89d4", "uri": "../unitgroups/54ccd2d9-a32a-4fc2-923d-f2c8c93e89d4"}}]}}, {"referenceToLCIAMethodDataSet": {"shortDescription": [{"value": "Potenzial für die Verknappung abiotischer Ressourcen – fossile Brennstoffe (ADPF)", "lang": "de"}, {"value": "Abiotic depletion potential - fossil resources (ADPF)", "lang": "en"}, {"value": "Abiotisk utarmningspotential av fossila resurser (ADP-F)", "lang": "sv"}], "type": "LCIA method data set", "refObjectId": "b2ad6110-c78d-11e6-9d9d-cec0c932ce01", "version": "01.00.012"}, "meanAmount": 0.0, "other": {"anies": [{"value": "26.3159665114842", "module": "A1", "scenario": "Standard scenario"}, {"value": "2.58342505505243", "module": "A2", "scenario": "Standard scenario"}, {"value": "6.4771937354824", "module": "A3", "scenario": "Standard scenario"}, {"value": "1.40379677812352", "module": "A4", "scenario": "Standard scenario"}, {"value": "0.0227856155807062", "module": "A5", "scenario": "Standard scenario"}, {"value": "0.0", "module": "B1", "scenario": "Standard scenario"}, {"value": "0.0", "module": "B2", "scenario": "Standard scenario"}, {"value": "0.0", "module": "B3", "scenario": "Standard scenario"}, {"value": "0.0", "module": "B4", "scenario": "Standard scenario"}, {"value": "0.0", "module": "B5", "scenario": "Standard scenario"}, {"value": "0.0", "module": "B6", "scenario": "Standard scenario"}, {"value": "0.0", "module": "B7", "scenario": "Standard scenario"}, {"value": "0.0", "module": "C1", "scenario": "Standard scenario"}, {"value": "0.109227530338128", "module": "C2", "scenario": "Standard scenario"}, {"value": "0.3280313438125", "module": "C3", "scenario": "Standard scenario"}, {"value": "0.012193933399", "module": "C4", "scenario": "Standard scenario"}, {"value": "-8.66099007709876", "module": "D", "scenario": "Standard scenario"}, {"name": "referenceToUnitGroupDataSet", "value": {"shortDescription": [{"value": "MJ"}], "type": "unit group data set", "refObjectId": "93a60a57-a3c8-11da-a746-0800200c9a66", "uri": "../unitgroups/93a60a57-a3c8-11da-a746-0800200c9a66"}}]}}, {"referenceToLCIAMethodDataSet": {"shortDescription": [{"value": "Versauerungspotenzial, kumulierte Überschreitung (AP)", "lang": "de"}, {"value": "Acidification potential, Accumulated Exceedance (AP)", "lang": "en"}, {"value": "Försurningspotential på land och vatten (AP)", "lang": "sv"}], "type": "LCIA method data set", "refObjectId": "b5c611c6-def3-11e6-bf01-fe55135034f3", "version": "01.03.011", "uri": "http://lca.jrc.ec.europa.eu/lcainfohub/datasets/elcd/lciamethods/f6cbd466-253f-4145-a4bb-8dae7d266e89.xml"}, "meanAmount": 0.0, "other": {"anies": [{"value": "0.106670507160739", "module": "A1", "scenario": "Standard scenario"}, {"value": "9.172078484853E-4", "module": "A2", "scenario": "Standard scenario"}, {"value": "0.0156895718210655", "module": "A3", "scenario": "Standard scenario"}, {"value": "5.398260619148E-4", "module": "A4", "scenario": "Standard scenario"}, {"value": "3.00262137948E-5", "module": "A5", "scenario": "Standard scenario"}, {"value": "0.0", "module": "B1", "scenario": "Standard scenario"}, {"value": "0.0", "module": "B2", "scenario": "Standard scenario"}, {"value": "0.0", "module": "B3", "scenario": "Standard scenario"}, {"value": "0.0", "module": "B4", "scenario": "Standard scenario"}, {"value": "0.0", "module": "B5", "scenario": "Standard scenario"}, {"value": "0.0", "module": "B6", "scenario": "Standard scenario"}, {"value": "0.0", "module": "B7", "scenario": "Standard scenario"}, {"value": "0.0", "module": "C1", "scenario": "Standard scenario"}, {"value": "4.20031364041E-5", "module": "C2", "scenario": "Standard scenario"}, {"value": "2.862122095E-4", "module": "C3", "scenario": "Standard scenario"}, {"value": "3.9810754E-6", "module": "C4", "scenario": "Standard scenario"}, {"value": "-0.0286475441180875", "module": "D", "scenario": "Standard scenario"}, {"name": "referenceToUnitGroupDataSet", "value": {"shortDescription": [{"value": "mol H+ eqv."}], "type": "unit group data set", "refObjectId": "42e089ac-92bf-4bf2-8ca1-5fc40d18f2ed", "uri": "../unitgroups/42e089ac-92bf-4bf2-8ca1-5fc40d18f2ed"}}]}}, {"referenceToLCIAMethodDataSet": {"shortDescription": [{"value": "Eutrophierungspotenzial - Süßwasser (EP-freshwater)", "lang": "de"}, {"value": "Eutrophication potential - freshwater (EP-freshwater)", "lang": "en"}, {"value": "Övergödningspotential sötvatten (EP-fw)", "lang": "sv"}], "type": "LCIA method data set", "refObjectId": "b53ec18f-7377-4ad3-86eb-cc3f4f276b2b", "version": "01.00.012", "uri": "http://lca.jrc.ec.europa.eu/lcainfohub/datasets/elcd/lciamethods/a4630d5b-df2f-48ae-b3f2-5e5257606d68.xml"}, "meanAmount": 0.0, "other": {"anies": [{"value": "0.0012957091371881", "module": "A1", "scenario": "Standard scenario"}, {"value": "1.6728395749E-6", "module": "A2", "scenario": "Standard scenario"}, {"value": "2.01609363594E-4", "module": "A3", "scenario": "Standard scenario"}, {"value": "9.389337902E-7", "module": "A4", "scenario": "Standard scenario"}, {"value": "1.811183041E-7", "module": "A5", "scenario": "Standard scenario"}, {"value": "0.0", "module": "B1", "scenario": "Standard scenario"}, {"value": "0.0", "module": "B2", "scenario": "Standard scenario"}, {"value": "0.0", "module": "B3", "scenario": "Standard scenario"}, {"value": "0.0", "module": "B4", "scenario": "Standard scenario"}, {"value": "0.0", "module": "B5", "scenario": "Standard scenario"}, {"value": "0.0", "module": "B6", "scenario": "Standard scenario"}, {"value": "0.0", "module": "B7", "scenario": "Standard scenario"}, {"value": "0.0", "module": "C1", "scenario": "Standard scenario"}, {"value": "7.30571694E-8", "module": "C2", "scenario": "Standard scenario"}, {"value": "1.5863708805E-6", "module": "C3", "scenario": "Standard scenario"}, {"value": "5.975692E-9", "module": "C4", "scenario": "Standard scenario"}, {"value": "-2.283373549522E-4", "module": "D", "scenario": "Standard scenario"}, {"name": "referenceToUnitGroupDataSet", "value": {"shortDescription": [{"value": "kg P eqv."}], "type": "unit group data set", "refObjectId": "0429039d-a61d-4590-ba67-aa4a20a810a1", "uri": "../unitgroups/0429039d-a61d-4590-ba67-aa4a20a810a1"}}]}}, {"referenceToLCIAMethodDataSet": {"shortDescription": [{"value": "Eutrophierungspotenzial - Salzwasser (EP-marine)", "lang": "de"}, {"value": "Eutrophication potential - marine (EP-marine)", "lang": "en"}, {"value": "Övergödningspotential marin (EP-m)", "lang": "sv"}], "type": "LCIA method data set", "refObjectId": "b5c619fa-def3-11e6-bf01-fe55135034f3", "version": "02.00.012", "uri": "http://lca.jrc.ec.europa.eu/lcainfohub/datasets/elcd/lciamethods/5296e2be-060b-4e50-b033-d45f85f6ac92.xml"}, "meanAmount": 0.0, "other": {"anies": [{"value": "0.007102437378521", "module": "A1", "scenario": "Standard scenario"}, {"value": "3.117098540709E-4", "module": "A2", "scenario": "Standard scenario"}, {"value": "0.0011803571153004", "module": "A3", "scenario": "Standard scenario"}, {"value": "1.902217586872E-4", "module": "A4", "scenario": "Standard scenario"}, {"value": "8.0865970084E-6", "module": "A5", "scenario": "Standard scenario"}, {"value": "0.0", "module": "B1", "scenario": "Standard scenario"}, {"value": "0.0", "module": "B2", "scenario": "Standard scenario"}, {"value": "0.0", "module": "B3", "scenario": "Standard scenario"}, {"value": "0.0", "module": "B4", "scenario": "Standard scenario"}, {"value": "0.0", "module": "B5", "scenario": "Standard scenario"}, {"value": "0.0", "module": "B6", "scenario": "Standard scenario"}, {"value": "0.0", "module": "B7", "scenario": "Standard scenario"}, {"value": "0.0", "module": "C1", "scenario": "Standard scenario"}, {"value": "1.48008979945E-5", "module": "C2", "scenario": "Standard scenario"}, {"value": "6.4028338E-5", "module": "C3", "scenario": "Standard scenario"}, {"value": "1.50030305E-6", "module": "C4", "scenario": "Standard scenario"}, {"value": "-0.0026740376343663", "module": "D", "scenario": "Standard scenario"}, {"name": "referenceToUnitGroupDataSet", "value": {"shortDescription": [{"value": "kg N eqv."}], "type": "unit group data set", "refObjectId": "d05bb823-ecdf-4686-8c40-bf1d9257859f", "uri": "../unitgroups/d05bb823-ecdf-4686-8c40-bf1d9257859f"}}]}}, {"referenceToLCIAMethodDataSet": {"shortDescription": [{"value": "Eutrophierungspotenzial - Land (EP-terrestrial)", "lang": "de"}, {"value": "Eutrophication potential - terrestrial (EP-terrestrial)", "lang": "en"}, {"value": "Övergödningspotential total (EP-T)", "lang": "sv"}], "type": "LCIA method data set", "refObjectId": "b5c614d2-def3-11e6-bf01-fe55135034f3", "version": "01.02.011", "uri": "http://lca.jrc.ec.europa.eu/lcainfohub/datasets/elcd/lciamethods/40054970-5936-477c-9bec-29fa23b1cb77.xml"}, "meanAmount": 0.0, "other": {"anies": [{"value": "0.103888432513344", "module": "A1", "scenario": "Standard scenario"}, {"value": "0.0034390019099305", "module": "A2", "scenario": "Standard scenario"}, {"value": "0.0157366095740338", "module": "A3", "scenario": "Standard scenario"}, {"value": "0.0020972171053241", "module": "A4", "scenario": "Standard scenario"}, {"value": "9.37777252839E-5", "module": "A5", "scenario": "Standard scenario"}, {"value": "0.0", "module": "B1", "scenario": "Standard scenario"}, {"value": "0.0", "module": "B2", "scenario": "Standard scenario"}, {"value": "0.0", "module": "B3", "scenario": "Standard scenario"}, {"value": "0.0", "module": "B4", "scenario": "Standard scenario"}, {"value": "0.0", "module": "B5", "scenario": "Standard scenario"}, {"value": "0.0", "module": "B6", "scenario": "Standard scenario"}, {"value": "0.0", "module": "B7", "scenario": "Standard scenario"}, {"value": "0.0", "module": "C1", "scenario": "Standard scenario"}, {"value": "1.631816289703E-4", "module": "C2", "scenario": "Standard scenario"}, {"value": "7.420022605E-4", "module": "C3", "scenario": "Standard scenario"}, {"value": "1.623958E-5", "module": "C4", "scenario": "Standard scenario"}, {"value": "-0.0413134337169505", "module": "D", "scenario": "Standard scenario"}, {"name": "referenceToUnitGroupDataSet", "value": {"shortDescription": [{"value": "mol N eqv."}], "type": "unit group data set", "refObjectId": "71b4d617-0ec9-4d3f-b65e-e438940c2401", "uri": "../unitgroups/71b4d617-0ec9-4d3f-b65e-e438940c2401"}}]}}, {"referenceToLCIAMethodDataSet": {"shortDescription": [{"value": "Globales Erwärmungspotenzial - total (GWP-total)", "lang": "de"}, {"value": "Global Warming Potential - total (GWP-total)", "lang": "en"}, {"value": "Global uppvärmningspotential – Totalt (GWP-T)", "lang": "sv"}], "type": "LCIA method data set", "refObjectId": "6a37f984-a4b3-458a-a20a-64418c145fa2", "version": "04.00.018"}, "meanAmount": 0.0, "other": {"anies": [{"value": "2.04887377304878", "module": "A1", "scenario": "Standard scenario"}, {"value": "0.171368940022783", "module": "A2", "scenario": "Standard scenario"}, {"value": "0.528104850895352", "module": "A3", "scenario": "Standard scenario"}, {"value": "0.0931547625558335", "module": "A4", "scenario": "Standard scenario"}, {"value": "0.0772933567010009", "module": "A5", "scenario": "Standard scenario"}, {"value": "0.0", "module": "B1", "scenario": "Standard scenario"}, {"value": "0.0", "module": "B2", "scenario": "Standard scenario"}, {"value": "0.0", "module": "B3", "scenario": "Standard scenario"}, {"value": "0.0", "module": "B4", "scenario": "Standard scenario"}, {"value": "0.0", "module": "B5", "scenario": "Standard scenario"}, {"value": "0.0", "module": "B6", "scenario": "Standard scenario"}, {"value": "0.0", "module": "B7", "scenario": "Standard scenario"}, {"value": "0.0", "module": "C1", "scenario": "Standard scenario"}, {"value": "0.0072482461933056", "module": "C2", "scenario": "Standard scenario"}, {"value": "0.057784747259", "module": "C3", "scenario": "Standard scenario"}, {"value": "6.60587327E-4", "module": "C4", "scenario": "Standard scenario"}, {"value": "-0.673101991976639", "module": "D", "scenario": "Standard scenario"}, {"name": "referenceToUnitGroupDataSet", "value": {"shortDescription": [{"value": "kg CO2-Äqv."}], "type": "unit group data set", "refObjectId": "1ebf3012-d0db-4de2-aefd-ef30cedb0be1", "uri": "../unitgroups/1ebf3012-d0db-4de2-aefd-ef30cedb0be1"}}]}}, {"referenceToLCIAMethodDataSet": {"shortDescription": [{"value": "Globales Erwärmungspotenzial - fossil (GWP-fossil)", "lang": "de"}, {"value": "Global Warming Potential - fossil fuels (GWP-fossil)", "lang": "en"}, {"value": "Global uppvärmningspotential– fossil (GWP-f)", "lang": "sv"}], "type": "LCIA method data set", "refObjectId": "5f635281-343e-44fb-83df-1971b155e6b6", "version": "01.00.011"}, "meanAmount": 0.0, "other": {"anies": [{"value": "2.0485776285908", "module": "A1", "scenario": "Standard scenario"}, {"value": "0.171225453393897", "module": "A2", "scenario": "Standard scenario"}, {"value": "0.578558507771495", "module": "A3", "scenario": "Standard scenario"}, {"value": "0.0930776865529617", "module": "A4", "scenario": "Standard scenario"}, {"value": "0.003834583230954", "module": "A5", "scenario": "Standard scenario"}, {"value": "0.0", "module": "B1", "scenario": "Standard scenario"}, {"value": "0.0", "module": "B2", "scenario": "Standard scenario"}, {"value": "0.0", "module": "B3", "scenario": "Standard scenario"}, {"value": "0.0", "module": "B4", "scenario": "Standard scenario"}, {"value": "0.0", "module": "B5", "scenario": "Standard scenario"}, {"value": "0.0", "module": "B6", "scenario": "Standard scenario"}, {"value": "0.0", "module": "B7", "scenario": "Standard scenario"}, {"value": "0.0", "module": "C1", "scenario": "Standard scenario"}, {"value": "0.0072422490136759", "module": "C2", "scenario": "Standard scenario"}, {"value": "0.059082691804", "module": "C3", "scenario": "Standard scenario"}, {"value": "6.398551205E-4", "module": "C4", "scenario": "Standard scenario"}, {"value": "-0.670746207193747", "module": "D", "scenario": "Standard scenario"}, {"name": "referenceToUnitGroupDataSet", "value": {"shortDescription": [{"value": "kg CO2-Äqv."}], "type": "unit group data set", "refObjectId": "1ebf3012-d0db-4de2-aefd-ef30cedb0be1", "uri": "../unitgroups/1ebf3012-d0db-4de2-aefd-ef30cedb0be1"}}]}}, {"referenceToLCIAMethodDataSet": {"shortDescription": [{"value": "Globales Erwärmungspotenzial - biogen (GWP-biogenic)", "lang": "de"}, {"value": "Global Warming Potential - biogenic (GWP-biogenic)", "lang": "en"}, {"value": "Global uppvärmningspotential – biogen (GWP-b)", "lang": "sv"}], "type": "LCIA method data set", "refObjectId": "2356e1ab-0185-4db5-86e5-16de51c7485c", "version": "01.00.007"}, "meanAmount": 0.0, "other": {"anies": [{"value": "-0.0018264604927606", "module": "A1", "scenario": "Standard scenario"}, {"value": "8.10159831704E-5", "module": "A2", "scenario": "Standard scenario"}, {"value": "-0.0523178869180237", "module": "A3", "scenario": "Standard scenario"}, {"value": "4.29692004882E-5", "module": "A4", "scenario": "Standard scenario"}, {"value": "0.0734576838625855", "module": "A5", "scenario": "Standard scenario"}, {"value": "0.0", "module": "B1", "scenario": "Standard scenario"}, {"value": "0.0", "module": "B2", "scenario": "Standard scenario"}, {"value": "0.0", "module": "B3", "scenario": "Standard scenario"}, {"value": "0.0", "module": "B4", "scenario": "Standard scenario"}, {"value": "0.0", "module": "B5", "scenario": "Standard scenario"}, {"value": "0.0", "module": "B6", "scenario": "Standard scenario"}, {"value": "0.0", "module": "B7", "scenario": "Standard scenario"}, {"value": "0.0", "module": "C1", "scenario": "Standard scenario"}, {"value": "3.3433754252E-6", "module": "C2", "scenario": "Standard scenario"}, {"value": "-0.001319799869", "module": "C3", "scenario": "Standard scenario"}, {"value": "2.06255515E-5", "module": "C4", "scenario": "Standard scenario"}, {"value": "-0.0016868618614895", "module": "D", "scenario": "Standard scenario"}, {"name": "referenceToUnitGroupDataSet", "value": {"shortDescription": [{"value": "kg CO2-Äqv."}], "type": "unit group data set", "refObjectId": "1ebf3012-d0db-4de2-aefd-ef30cedb0be1", "uri": "../unitgroups/1ebf3012-d0db-4de2-aefd-ef30cedb0be1"}}]}}, {"referenceToLCIAMethodDataSet": {"shortDescription": [{"value": "Globales Erwärmungspotenzial - luluc (GWP-luluc)", "lang": "de"}, {"value": "Global Warming Potential - land use and land use change (GWP-luluc)", "lang": "en"}, {"value": "Global uppvärmningspotential - markanvändning och förändringar i markanvändning (GWP-luluc)", "lang": "sv"}], "type": "LCIA method data set", "refObjectId": "4331bbdb-978a-490d-8707-eeb047f01a55", "version": "01.00.007"}, "meanAmount": 0.0, "other": {"anies": [{"value": "0.0021226049507405", "module": "A1", "scenario": "Standard scenario"}, {"value": "6.24706457165E-5", "module": "A2", "scenario": "Standard scenario"}, {"value": "0.0019893480012763", "module": "A3", "scenario": "Standard scenario"}, {"value": "3.41068023836E-5", "module": "A4", "scenario": "Standard scenario"}, {"value": "1.1129944881E-6", "module": "A5", "scenario": "Standard scenario"}, {"value": "0.0", "module": "B1", "scenario": "Standard scenario"}, {"value": "0.0", "module": "B2", "scenario": "Standard scenario"}, {"value": "0.0", "module": "B3", "scenario": "Standard scenario"}, {"value": "0.0", "module": "B4", "scenario": "Standard scenario"}, {"value": "0.0", "module": "B5", "scenario": "Standard scenario"}, {"value": "0.0", "module": "B6", "scenario": "Standard scenario"}, {"value": "0.0", "module": "B7", "scenario": "Standard scenario"}, {"value": "0.0", "module": "C1", "scenario": "Standard scenario"}, {"value": "2.6538042045E-6", "module": "C2", "scenario": "Standard scenario"}, {"value": "2.617254985E-5", "module": "C3", "scenario": "Standard scenario"}, {"value": "1.3129738E-7", "module": "C4", "scenario": "Standard scenario"}, {"value": "-6.689208209505E-4", "module": "D", "scenario": "Standard scenario"}, {"name": "referenceToUnitGroupDataSet", "value": {"shortDescription": [{"value": "kg CO2-Äqv."}], "type": "unit group data set", "refObjectId": "1ebf3012-d0db-4de2-aefd-ef30cedb0be1", "uri": "../unitgroups/1ebf3012-d0db-4de2-aefd-ef30cedb0be1"}}]}}, {"referenceToLCIAMethodDataSet": {"shortDescription": [{"value": "Abbaupotenzial der stratosphärischen Ozonschicht (ODP)", "lang": "de"}, {"value": "Depletion potential of the stratospheric ozone layer (ODP)", "lang": "en"}, {"value": "Utarmningspotential för stratosfäriska ozonskiktet - ozonnedbrytning (ODP)", "lang": "sv"}], "type": "LCIA method data set", "refObjectId": "b5c629d6-def3-11e6-bf01-fe55135034f3", "version": "02.00.014", "uri": "http://lca.jrc.ec.europa.eu/lcainfohub/datasets/elcd/lciamethods/8b723200-3d8f-4eec-9e10-444edb029476.xml"}, "meanAmount": 0.0, "other": {"anies": [{"value": "1.430161262E-7", "module": "A1", "scenario": "Standard scenario"}, {"value": "3.79683803E-8", "module": "A2", "scenario": "Standard scenario"}, {"value": "5.31959798E-8", "module": "A3", "scenario": "Standard scenario"}, {"value": "2.05444808E-8", "module": "A4", "scenario": "Standard scenario"}, {"value": "3.322263E-10", "module": "A5", "scenario": "Standard scenario"}, {"value": "0.0", "module": "B1", "scenario": "Standard scenario"}, {"value": "0.0", "module": "B2", "scenario": "Standard scenario"}, {"value": "0.0", "module": "B3", "scenario": "Standard scenario"}, {"value": "0.0", "module": "B4", "scenario": "Standard scenario"}, {"value": "0.0", "module": "B5", "scenario": "Standard scenario"}, {"value": "0.0", "module": "B6", "scenario": "Standard scenario"}, {"value": "0.0", "module": "B7", "scenario": "Standard scenario"}, {"value": "0.0", "module": "C1", "scenario": "Standard scenario"}, {"value": "1.5985383E-9", "module": "C2", "scenario": "Standard scenario"}, {"value": "3.4130057E-9", "module": "C3", "scenario": "Standard scenario"}, {"value": "1.637161E-10", "module": "C4", "scenario": "Standard scenario"}, {"value": "-5.40167548E-8", "module": "D", "scenario": "Standard scenario"}, {"name": "referenceToUnitGroupDataSet", "value": {"shortDescription": [{"value": "kg CFC 11-Äquiv."}], "type": "unit group data set", "refObjectId": "d9e957c9-7309-4474-bf3a-7777df6c4e5b", "uri": "../unitgroups/d9e957c9-7309-4474-bf3a-7777df6c4e5b"}}]}}, {"referenceToLCIAMethodDataSet": {"shortDescription": [{"value": "Bildungspotenzial für troposphärisches Ozon (POCP)", "lang": "de"}, {"value": "Photochemical Ozone Creation Potential (POCP)", "lang": "en"}, {"value": "Potential till fotokemisk oxidantbildning – marknära ozon (POCP)", "lang": "sv"}], "type": "LCIA method data set", "refObjectId": "b5c610fe-def3-11e6-bf01-fe55135034f3", "version": "02.00.017", "uri": "http://lca.jrc.ec.europa.eu/lcainfohub/datasets/elcd/lciamethods/ec7836be-83eb-41da-bcda-1a6a3fe2d149.xml"}, "meanAmount": 0.0, "other": {"anies": [{"value": "0.0257867183687555", "module": "A1", "scenario": "Standard scenario"}, {"value": "9.979399477856E-4", "module": "A2", "scenario": "Standard scenario"}, {"value": "0.0043140994113171", "module": "A3", "scenario": "Standard scenario"}, {"value": "5.987705881124E-4", "module": "A4", "scenario": "Standard scenario"}, {"value": "2.5051868034E-5", "module": "A5", "scenario": "Standard scenario"}, {"value": "0.0", "module": "B1", "scenario": "Standard scenario"}, {"value": "0.0", "module": "B2", "scenario": "Standard scenario"}, {"value": "0.0", "module": "B3", "scenario": "Standard scenario"}, {"value": "0.0", "module": "B4", "scenario": "Standard scenario"}, {"value": "0.0", "module": "B5", "scenario": "Standard scenario"}, {"value": "0.0", "module": "B6", "scenario": "Standard scenario"}, {"value": "0.0", "module": "B7", "scenario": "Standard scenario"}, {"value": "0.0", "module": "C1", "scenario": "Standard scenario"}, {"value": "4.6589530335E-5", "module": "C2", "scenario": "Standard scenario"}, {"value": "2.019487085E-4", "module": "C3", "scenario": "Standard scenario"}, {"value": "4.6822033E-6", "module": "C4", "scenario": "Standard scenario"}, {"value": "-0.0090917867614826", "module": "D", "scenario": "Standard scenario"}, {"name": "referenceToUnitGroupDataSet", "value": {"shortDescription": [{"value": "kg NMVOC eqv."}], "type": "unit group data set", "refObjectId": "d27c25f8-fbc1-44c6-b47b-4adbae4199c6", "uri": "../unitgroups/d27c25f8-fbc1-44c6-b47b-4adbae4199c6"}}]}}, {"referenceToLCIAMethodDataSet": {"shortDescription": [{"value": "Wasser-Entzugspotenzial (Benutzer) (WDP)", "lang": "de"}, {"value": "Water (user) deprivation potential (WDP)", "lang": "en"}, {"value": "Vattenfotavtryck (WDP)", "lang": "sv"}], "type": "LCIA method data set", "refObjectId": "b2ad66ce-c78d-11e6-9d9d-cec0c932ce01", "version": "03.00.016"}, "meanAmount": 0.0, "other": {"anies": [{"value": "1.27252914430366", "module": "A1", "scenario": "Standard scenario"}, {"value": "0.0089499392664834", "module": "A2", "scenario": "Standard scenario"}, {"value": "0.168656057875415", "module": "A3", "scenario": "Standard scenario"}, {"value": "0.0050223564106969", "module": "A4", "scenario": "Standard scenario"}, {"value": "4.673142609302E-4", "module": "A5", "scenario": "Standard scenario"}, {"value": "0.0", "module": "B1", "scenario": "Standard scenario"}, {"value": "0.0", "module": "B2", "scenario": "Standard scenario"}, {"value": "0.0", "module": "B3", "scenario": "Standard scenario"}, {"value": "0.0", "module": "B4", "scenario": "Standard scenario"}, {"value": "0.0", "module": "B5", "scenario": "Standard scenario"}, {"value": "0.0", "module": "B6", "scenario": "Standard scenario"}, {"value": "0.0", "module": "B7", "scenario": "Standard scenario"}, {"value": "0.0", "module": "C1", "scenario": "Standard scenario"}, {"value": "3.90782765545E-4", "module": "C2", "scenario": "Standard scenario"}, {"value": "0.0036958938655", "module": "C3", "scenario": "Standard scenario"}, {"value": "7.02042385E-5", "module": "C4", "scenario": "Standard scenario"}, {"value": "-0.572852380164492", "module": "D", "scenario": "Standard scenario"}, {"name": "referenceToUnitGroupDataSet", "value": {"shortDescription": [{"value": "m3 world eqv."}], "type": "unit group data set", "refObjectId": "6ae2df01-888e-46c8-b17d-49fa3869b476", "uri": "../unitgroups/6ae2df01-888e-46c8-b17d-49fa3869b476"}}]}}, {"referenceToLCIAMethodDataSet": {"shortDescription": [{"value": "Potenzielles Auftreten von Krankheiten aufgrund von Feinstaubemissionen (PM)", "lang": "de"}, {"value": "Potential incidence of disease due to PM emissions (PM)", "lang": "en"}, {"value": "Potential till utsläpp av partiklar (PM)", "lang": "sv"}], "type": "LCIA method data set", "refObjectId": "b5c602c6-def3-11e6-bf01-fe55135034f3", "version": "02.00.013", "uri": "http://lca.jrc.ec.europa.eu/lcainfohub/datasets/elcd/lciamethods/72ce3013-f678-4c6a-935b-f4752ff8901b.xml"}, "meanAmount": 0.0, "other": {"anies": [{"value": "2.973997446E-7", "module": "A1", "scenario": "Standard scenario"}, {"value": "1.47226375E-8", "module": "A2", "scenario": "Standard scenario"}, {"value": "5.68278165E-8", "module": "A3", "scenario": "Standard scenario"}, {"value": "8.3736029E-9", "module": "A4", "scenario": "Standard scenario"}, {"value": "2.17471E-10", "module": "A5", "scenario": "Standard scenario"}, {"value": "0.0", "module": "B1", "scenario": "Standard scenario"}, {"value": "0.0", "module": "B2", "scenario": "Standard scenario"}, {"value": "0.0", "module": "B3", "scenario": "Standard scenario"}, {"value": "0.0", "module": "B4", "scenario": "Standard scenario"}, {"value": "0.0", "module": "B5", "scenario": "Standard scenario"}, {"value": "0.0", "module": "B6", "scenario": "Standard scenario"}, {"value": "0.0", "module": "B7", "scenario": "Standard scenario"}, {"value": "0.0", "module": "C1", "scenario": "Standard scenario"}, {"value": "6.515387E-10", "module": "C2", "scenario": "Standard scenario"}, {"value": "3.5620907E-9", "module": "C3", "scenario": "Standard scenario"}, {"value": "8.17445E-11", "module": "C4", "scenario": "Standard scenario"}, {"value": "-1.027003418E-7", "module": "D", "scenario": "Standard scenario"}, {"name": "referenceToUnitGroupDataSet", "value": {"shortDescription": [{"value": "disease incidence"}], "type": "unit group data set", "refObjectId": "3883559b-648f-4afc-8ba2-0bd24f3affa3", "uri": "../unitgroups/3883559b-648f-4afc-8ba2-0bd24f3affa3"}}]}}, {"referenceToLCIAMethodDataSet": {"shortDescription": [{"value": "Potenzielle Wirkung durch Exposition des Menschen mit U235 (IRP)", "lang": "de"}, {"value": "Potential Human exposure efficiency relative to U235 (IRP)", "lang": "en"}, {"value": "Exponeringseffektivitet relaterad till U235 (IR)", "lang": "sv"}], "type": "LCIA method data set", "refObjectId": "b5c632be-def3-11e6-bf01-fe55135034f3", "version": "01.00.013", "uri": "http://lca.jrc.ec.europa.eu/lcainfohub/datasets/elcd/lciamethods/a6f4cbc8-5388-44d6-9a67-53d05684f93e.xml"}, "meanAmount": 0.0, "other": {"anies": [{"value": "0.115644690479845", "module": "A1", "scenario": "Standard scenario"}, {"value": "0.0108949916606066", "module": "A2", "scenario": "Standard scenario"}, {"value": "0.0290725425494888", "module": "A3", "scenario": "Standard scenario"}, {"value": "0.00588170331566", "module": "A4", "scenario": "Standard scenario"}, {"value": "9.44977601284E-5", "module": "A5", "scenario": "Standard scenario"}, {"value": "0.0", "module": "B1", "scenario": "Standard scenario"}, {"value": "0.0", "module": "B2", "scenario": "Standard scenario"}, {"value": "0.0", "module": "B3", "scenario": "Standard scenario"}, {"value": "0.0", "module": "B4", "scenario": "Standard scenario"}, {"value": "0.0", "module": "B5", "scenario": "Standard scenario"}, {"value": "0.0", "module": "B6", "scenario": "Standard scenario"}, {"value": "0.0", "module": "B7", "scenario": "Standard scenario"}, {"value": "0.0", "module": "C1", "scenario": "Standard scenario"}, {"value": "4.576473869743E-4", "module": "C2", "scenario": "Standard scenario"}, {"value": "0.001617969456", "module": "C3", "scenario": "Standard scenario"}, {"value": "6.04591075E-5", "module": "C4", "scenario": "Standard scenario"}, {"value": "-0.040414369092105", "module": "D", "scenario": "Standard scenario"}, {"name": "referenceToUnitGroupDataSet", "value": {"shortDescription": [{"value": "kBq U235 eqv."}], "type": "unit group data set", "refObjectId": "456b05bf-1415-44a9-9993-02452f554c09", "uri": "../unitgroups/456b05bf-1415-44a9-9993-02452f554c09"}}]}}, {"referenceToLCIAMethodDataSet": {"shortDescription": [{"value": "Potenzielle Toxizitätsvergleichseinheit für Ökosysteme (ETP-fw)", "lang": "de"}, {"value": "Potential Comparative Toxic Unit for ecosystems (ETP-fw)", "lang": "en"}, {"value": "Ecotoxicitet (ETP-fw) ", "lang": "sv"}], "type": "LCIA method data set", "refObjectId": "ee1082d1-b0f7-43ca-a1f0-21e2a4a74511", "version": "01.00.004", "uri": "http://lca.jrc.ec.europa.eu/lcainfohub/datasets/elcd/lciamethods/ee1082d1-b0f7-43ca-a1f0-21e2a4a74511.xml"}, "meanAmount": 0.0, "other": {"anies": [{"value": "1333.99751253084", "module": "A1", "scenario": "Standard scenario"}, {"value": "2.26989754032119", "module": "A2", "scenario": "Standard scenario"}, {"value": "159.577767177578", "module": "A3", "scenario": "Standard scenario"}, {"value": "1.25179524333649", "module": "A4", "scenario": "Standard scenario"}, {"value": "0.209556549523128", "module": "A5", "scenario": "Standard scenario"}, {"value": "0.0", "module": "B1", "scenario": "Standard scenario"}, {"value": "0.0", "module": "B2", "scenario": "Standard scenario"}, {"value": "0.0", "module": "B3", "scenario": "Standard scenario"}, {"value": "0.0", "module": "B4", "scenario": "Standard scenario"}, {"value": "0.0", "module": "B5", "scenario": "Standard scenario"}, {"value": "0.0", "module": "B6", "scenario": "Standard scenario"}, {"value": "0.0", "module": "B7", "scenario": "Standard scenario"}, {"value": "0.0", "module": "C1", "scenario": "Standard scenario"}, {"value": "0.0974004963178729", "module": "C2", "scenario": "Standard scenario"}, {"value": "1.43977675611049", "module": "C3", "scenario": "Standard scenario"}, {"value": "0.057566008629", "module": "C4", "scenario": "Standard scenario"}, {"value": "-510.550741592322", "module": "D", "scenario": "Standard scenario"}, {"name": "referenceToUnitGroupDataSet", "value": {"shortDescription": [{"value": "CTUe"}], "type": "unit group data set", "refObjectId": "aa959ded-f1eb-4efb-9c5c-2d60be36b3e6", "uri": "../unitgroups/aa959ded-f1eb-4efb-9c5c-2d60be36b3e6"}}]}}, {"referenceToLCIAMethodDataSet": {"shortDescription": [{"value": "Potenzielle Toxizitätsvergleichseinheit für den Menschen - kanzerogene Wirkung (HTP-c)", "lang": "de"}, {"value": "Potential Comparative Toxic Unit for humans - cancer effects (HTP-c)", "lang": "en"}, {"value": "Humantoxicitet – cancer (HTP-c)", "lang": "sv"}], "type": "LCIA method data set", "refObjectId": "2299222a-bbd8-474f-9d4f-4dd1f18aea7c", "version": "01.00.005", "uri": "http://lca.jrc.ec.europa.eu/lcainfohub/datasets/elcd/lciamethods/2299222a-bbd8-474f-9d4f-4dd1f18aea7c.xml"}, "meanAmount": 0.0, "other": {"anies": [{"value": "1.9464676E-8", "module": "A1", "scenario": "Standard scenario"}, {"value": "7.2173E-11", "module": "A2", "scenario": "Standard scenario"}, {"value": "1.9199229E-9", "module": "A3", "scenario": "Standard scenario"}, {"value": "4.06013E-11", "module": "A4", "scenario": "Standard scenario"}, {"value": "1.33145E-11", "module": "A5", "scenario": "Standard scenario"}, {"value": "0.0", "module": "B1", "scenario": "Standard scenario"}, {"value": "0.0", "module": "B2", "scenario": "Standard scenario"}, {"value": "0.0", "module": "B3", "scenario": "Standard scenario"}, {"value": "0.0", "module": "B4", "scenario": "Standard scenario"}, {"value": "0.0", "module": "B5", "scenario": "Standard scenario"}, {"value": "0.0", "module": "B6", "scenario": "Standard scenario"}, {"value": "0.0", "module": "B7", "scenario": "Standard scenario"}, {"value": "0.0", "module": "C1", "scenario": "Standard scenario"}, {"value": "3.1591E-12", "module": "C2", "scenario": "Standard scenario"}, {"value": "3.4188E-11", "module": "C3", "scenario": "Standard scenario"}, {"value": "5.569E-13", "module": "C4", "scenario": "Standard scenario"}, {"value": "-1.11581287E-8", "module": "D", "scenario": "Standard scenario"}, {"name": "referenceToUnitGroupDataSet", "value": {"shortDescription": [{"value": "CTUh"}], "type": "unit group data set", "refObjectId": "d4c9523e-2d7e-49fd-8469-998f547d3a70", "uri": "../unitgroups/d4c9523e-2d7e-49fd-8469-998f547d3a70"}}]}}, {"referenceToLCIAMethodDataSet": {"shortDescription": [{"value": "Potenzielle Toxizitätsvergleichseinheit für den Menschen - nicht kanzerogene Wirkung (HTP-nc)", "lang": "de"}, {"value": "Potential Comparative Toxic Unit for humans - non-cancer effects (HTP-nc)", "lang": "en"}, {"value": "Humantoxicitet – icke cancer (HTP-nc)", "lang": "sv"}], "type": "LCIA method data set", "refObjectId": "3af763a5-b7a1-48c9-9cee-1f223481fcef", "version": "01.00.004", "uri": "http://lca.jrc.ec.europa.eu/lcainfohub/datasets/elcd/lciamethods/3af763a5-b7a1-48c9-9cee-1f223481fcef.xml"}, "meanAmount": 0.0, "other": {"anies": [{"value": "1.5537735129E-6", "module": "A1", "scenario": "Standard scenario"}, {"value": "2.4702262E-9", "module": "A2", "scenario": "Standard scenario"}, {"value": "1.411255227E-7", "module": "A3", "scenario": "Standard scenario"}, {"value": "1.3692759E-9", "module": "A4", "scenario": "Standard scenario"}, {"value": "2.397681E-10", "module": "A5", "scenario": "Standard scenario"}, {"value": "0.0", "module": "B1", "scenario": "Standard scenario"}, {"value": "0.0", "module": "B2", "scenario": "Standard scenario"}, {"value": "0.0", "module": "B3", "scenario": "Standard scenario"}, {"value": "0.0", "module": "B4", "scenario": "Standard scenario"}, {"value": "0.0", "module": "B5", "scenario": "Standard scenario"}, {"value": "0.0", "module": "B6", "scenario": "Standard scenario"}, {"value": "0.0", "module": "B7", "scenario": "Standard scenario"}, {"value": "0.0", "module": "C1", "scenario": "Standard scenario"}, {"value": "1.065415E-10", "module": "C2", "scenario": "Standard scenario"}, {"value": "1.6216683E-9", "module": "C3", "scenario": "Standard scenario"}, {"value": "4.50273E-11", "module": "C4", "scenario": "Standard scenario"}, {"value": "-8.110842918E-7", "module": "D", "scenario": "Standard scenario"}, {"name": "referenceToUnitGroupDataSet", "value": {"shortDescription": [{"value": "CTUh"}], "type": "unit group data set", "refObjectId": "d4c9523e-2d7e-49fd-8469-998f547d3a70", "uri": "../unitgroups/d4c9523e-2d7e-49fd-8469-998f547d3a70"}}]}}, {"referenceToLCIAMethodDataSet": {"shortDescription": [{"value": "Potenzieller Bodenqualitätsindex (SQP)", "lang": "de"}, {"value": "Potential Soil quality index (SQP)", "lang": "en"}, {"value": "Potentiell jordkvalitet index (SQP)", "lang": "sv"}], "type": "LCIA method data set", "refObjectId": "b2ad6890-c78d-11e6-9d9d-cec0c932ce01", "version": "01.00.014"}, "meanAmount": 0.0, "other": {"anies": [{"value": "27.2848542636653", "module": "A1", "scenario": "Standard scenario"}, {"value": "2.1746600127366", "module": "A2", "scenario": "Standard scenario"}, {"value": "19.2714075930984", "module": "A3", "scenario": "Standard scenario"}, {"value": "1.21743197375421", "module": "A4", "scenario": "Standard scenario"}, {"value": "0.0188480608386771", "module": "A5", "scenario": "Standard scenario"}, {"value": "0.0", "module": "B1", "scenario": "Standard scenario"}, {"value": "0.0", "module": "B2", "scenario": "Standard scenario"}, {"value": "0.0", "module": "B3", "scenario": "Standard scenario"}, {"value": "0.0", "module": "B4", "scenario": "Standard scenario"}, {"value": "0.0", "module": "B5", "scenario": "Standard scenario"}, {"value": "0.0", "module": "B6", "scenario": "Standard scenario"}, {"value": "0.0", "module": "B7", "scenario": "Standard scenario"}, {"value": "0.0", "module": "C1", "scenario": "Standard scenario"}, {"value": "0.0947267367471795", "module": "C2", "scenario": "Standard scenario"}, {"value": "0.6491172637705", "module": "C3", "scenario": "Standard scenario"}, {"value": "0.029834691802", "module": "C4", "scenario": "Standard scenario"}, {"value": "-11.8617945580632", "module": "D", "scenario": "Standard scenario"}, {"name": "referenceToUnitGroupDataSet", "value": {"shortDescription": [{"value": "dimensionless"}], "type": "unit group data set", "refObjectId": "f130951c-e67f-4f7f-8dd4-665de3974e18", "uri": "../unitgroups/f130951c-e67f-4f7f-8dd4-665de3974e18"}}]}}]}, "otherAttributes": {"{http://www.okworx.com/ILCD/Extensions/2018/Profile}profile": "EN_15804_A2", "{http://www.indata.network/EPD/2019}epd-version": "1.2"}, "version": "1.1"}