{"processInformation": {"dataSetInformation": {"UUID": "b452a1d8-b252-4f3b-914d-1b19bd268a2e", "name": {"baseName": [{"value": "RAVATHERM™ XPS (X) extruded polystyrene foam insulation with non-halogenated blowing agents", "lang": "en"}, {"value": "RAVATHERM™ XPS (X) Isolierung aus extrudiertem Polystyrolschaum mit halogenfreiem Treibmittel", "lang": "de"}], "functionalUnitFlowProperties": [{"lang": "en"}]}, "classificationInformation": {"classification": [{"class": [{"value": "Dämmstoffe", "level": 0, "classId": "2"}, {"value": "Extrudiertes Polystyrol (XPS)", "level": 1, "classId": "2.3"}, {"value": "XPS weiß", "level": 2, "classId": "2.3.01"}], "name": "OEKOBAU.DAT"}, {"class": [{"value": "02 Building products", "level": 0}, {"value": "Thermal insulation products", "level": 1}, {"value": "Insulating materials made of foam plastics", "level": 2}], "name": "IBUCategories"}]}, "generalComment": [{"value": "RAVATHERM(TM) XPS and XPS X extruded polystyrene foams (XPS) are thermoplastic insulation foams produced according to EN 13164 Building insulation, EN 14307 Equipment insulation. \n\nThey are available in blue or grey board shape with a density range from 25 to 50 kg/m3. The boards can be delivered in various compressive strength values from 150 to 700 kPa. \nTo meet the need of various applications the boards are produced with different surfaces: with the extrusion skin, planed, grooved or with thermal embossing.\nThese XPS boards are supplied with different edge treatments such as butt edge, shiplap and tongue and groove. The EPD is related to unfaced XPS products only; Heat lamination of several XPS layers is included. Additional product treatment\nis not considered.", "lang": "en"}, {"value": "RAVATHERM(TM) XPS und XPS X extrudierte Polystyrol-Schaumstoffe (XPS) sind thermoplastische Dämmstoffe, die gemäß EN 13164 Gebäudeisolierung, EN 14307 Geräteisolierung hergestellt werden. \n\nSie sind in blauer oder grauer Plattenform mit einer Dichte von 25 bis 50 kg/m3 erhältlich. Die Platten können in verschiedenen Druckfestigkeiten von 150 bis 700 kPa geliefert werden. \nUm den Anforderungen der verschiedenen Anwendungen gerecht zu werden, werden die Platten mit verschiedenen Oberflächen hergestellt: mit der Extrusionshaut, gehobelt, gerillt oder mit thermischer Prägung. Diese XPS-Platten werden mit verschiedenen Kantenbehandlungen wie Stoßkante, Schiffslatte und Nut und Feder geliefert. Die EPD bezieht sich nur auf unbehandelte XPS-Produkte; die Wärmelaminierung mehrerer XPS-Schichten ist eingeschlossen. Eine zusätzliche Produktbehandlung wird nicht berücksichtigt.", "lang": "de"}], "other": {"anies": [{"scenario": [{"description": [{"value": "100% incineration", "lang": "en"}, {"value": "100% Verbrennung", "lang": "de"}], "name": "S1", "default": true}, {"description": [{"value": "100% landfill", "lang": "en"}, {"value": "100% Mülldeponie", "lang": "de"}], "name": "S2"}]}]}}, "quantitativeReference": {"referenceToReferenceFlow": [0]}, "time": {"referenceYear": 2023, "dataSetValidUntil": 2028, "other": {"anies": [{"name": "publicationDateOfEPD", "value": 1698710400000}]}}, "geography": {"locationOfOperationSupplyOrProduction": {"location": "RER"}}, "technology": {"technologyDescriptionAndIncludedProcesses": [{"value": "XPS is produced by a continuous extrusion process using electricity as the main power source: polystyrenegranules are melted in an extruder and a blowingagent is injected into the extruder under high pressure.The drop in pressure at the exit die causes thepolystyrene to foam into a board with homogeneousand closed cell structure.Then the boards’ edges are trimmed, and the productis cut to dimensions. The smooth foam skin resultingfrom the extrusion process remains on the boards or isremoved mechanically for particular board types toachieve better adhesive strength in combination withe.g. concrete, mortar, or construction adhesives. Someboards receive special surface patterns or grooves.Most of XPS foams off-grade material or scrap fromproduction is ground and extruded in a separate line,the resulting recycle is then used in the productionprocess of XPS. \nTechnical data: \nAcoustic properties are not relevant for XPS foams. \nFor fire performance, these products usually achieve the fire classification Euroclass E according to EN 13501-1. \nDeclared unit: \nThe declared unit is 1 m of the XPS insulation product. The declared product reflects the average of seven of Ravagos sites weighted by production volume share:\n\nBalaton (HU); 33.07 kg/m3 (18%)\nRheinmuenster (DE): 34.75 kg/m3 (18%)\nLavrion (GR): 33.60 kg/m3 (17%)\nSchkopau (DE): 35.23 kg/m3 (17%)\nDrusenheim (FR): 35.35 kg/m3 (16%)\nArtix (FR): 33.63 kg/m3 (9%)\nKings Lynn (GB): 38.08 kg/m3 (5%)\n\nThe weighted average density of the product is 34.4 kg/m.", "lang": "en"}, {"value": "XPS wird in einem kontinuierlichen Extrusionsverfahren hergestellt, bei dem Elektrizität als Hauptstromquelle verwendet wird: Polystyrolgranulate werden in einem Extruder geschmolzen und ein Treibmittel wird unter hohem Druck in den Extruder eingespritzt. Der Druckabfall an der Austrittsdüse lässt das Polystyrol zu einer Platte mit homogener und geschlossener Zellstruktur aufschäumen. Die glatte Schaumstoffhaut aus dem Extrusionsprozess verbleibt auf den Platten oder wird bei bestimmten Plattentypen mechanisch entfernt, um eine bessere Haftfestigkeit in Kombination mit z.B. Beton, Mörtel oder Konstruktionsklebstoffen zu erreichen. Einige Platten erhalten spezielle Oberflächenmuster oder Rillen. Der größte Teil der XPS-Schaumstoffe wird in einer separaten Linie gemahlen und extrudiert, das dabei anfallende Recyclingmaterial wird dann für die Herstellung von XPS verwendet. \nTechnische Daten: \nAkustische Eigenschaften sind für XPS-Schaumstoffe nicht relevant. \nWas das Brandverhalten betrifft, so erreichen diese Produkte in der Regel die Brandklasse E gemäß EN 13501-1. \nDeklarierte Einheit: \nDie angegebene Einheit ist 1 m³ des XPS-Dämmstoffs. Das angegebene Produkt spiegelt den Durchschnitt von sieben Ravago-Standorten wider, gewichtet nach dem Anteil der Produktionsmengen: Balaton (HU); 33,07 kg/m3 (18%) Rheinmünster (DE): 34,75 kg/m3 (18%) Lavrion (GR): 33,60 kg/m3 (17%) Schkopau (DE): 35,23 kg/m3 (17%) Drusenheim (FR): 35,35 kg/m3 (16%) Artix (FR): 33,63 kg/m3 (9%) King's Lynn (GB): 38,08 kg/m3 (5%) Die gewichtete durchschnittliche Dichte des Produkts beträgt 34,4 kg/m³.", "lang": "de"}], "technologicalApplicability": [{"value": "The variety of the performance properties of RAVATHERM XPS and XPS X thermal insulation foams make them suitable for use in a large number of applications such as: perimeter insulation, inverted insulation for terrace roofs, insulation of pitched roofs, floor insulation including insulation of highly loaded industrial floors, insulation of thermal bridges for exterior walls, External Thermal Insulation Composite System (ETICS), insulation of cavity walls, agricultural building ceiling insulation, prefabricated elements e.g. building sandwich panels, insulation for building equipment and industrial installations (pipe sections, ).", "lang": "en"}, {"value": "Die Vielfalt der Leistungseigenschaften von RAVATHERM XPS und XPS X Wärmedämmschaumstoffen macht sie für eine Vielzahl von Anwendungen geeignet, wie z.B.: Perimeterdämmung, Umkehrdämmung für Terrassendächer, Dämmung von Schrägdächern, Bodendämmung einschließlich der Dämmung von hochbelasteten Industrieböden, Dämmung von Wärmebrücken für Außenwände, Externes Wärmedämmverbundsystem (WDVS), Dämmung von Hohlwänden, Deckendämmung für landwirtschaftliche Gebäude, vorgefertigte Elemente wie z.B. Bausandwichpaneele, Dämmung von Baugeräten und Industrieanlagen (Rohrleitungsabschnitte, ...).", "lang": "de"}]}}, "modellingAndValidation": {"LCIMethodAndAllocation": {"typeOfDataSet": "EPD", "referenceToLCAMethodDetails": [{"shortDescription": [{"value": "Insulating materials made of foam plastics.pdf", "lang": "en"}], "type": "source data set", "refObjectId": "d36707fd-1eb0-4601-8a7c-20bdaa95418c"}], "other": {"anies": [{"name": "subType", "value": "average dataset"}]}}, "dataSourcesTreatmentAndRepresentativeness": {"referenceToDataSource": [{"shortDescription": [{"value": "GaBi Database (all versions)", "lang": "en"}], "type": "source data set", "refObjectId": "28d74cc0-db8b-4d7e-bc44-5f6d56ce0c4a"}, {"shortDescription": [{"value": "GaBi Database Edition 2022, CUP 2022.02", "lang": "en"}], "type": "source data set", "refObjectId": "94f442cb-662e-43ea-a792-4b0a35132e93"}], "useAdviceForDataSet": [{"value": "Scope: \nThe data have been provided by the seven ISO 14001 certified factories of Ravago Building Solutions producing these products in France, Germany, Greece, Hungary and the UK for the year 2021. \nSystem boundary: \nType of EPD according to EN 15804: \"cradle to gate with options, modules C1–C4, and module D\". The following modules are declared: A1A3, C, D and additional modules: A4 + A5. \n\nProduction - Modules A1-A3\nThe product stage includes:\n\nRaw material supply including secondary materials (A1)\n\nTransport to the manufacturer (A2): Transport is considered for all the input raw materials\nManufacturing (A3), including provision of all materials, products and energy, as well as waste processing up to the end-of-waste state.\nConstruction stage - Modules A4-A5\nThe construction process stage includes:\n\nTransport to the construction site (A4)\n\nTreatment of packaging material (A5)\nEnd-of-life stage Modules C1-C4 and D\nThe end-of-life stage includes\n\nManual dismantling (Load free) (C1)\n\nTransport to EoL (C2)\n\nWaste processing & disposal (C) with two 100 % scenarios (scenario 1: Incineration (C3 and D); scenario 2: Landfill (C4))\n\nReuse, recovery or recycling potential (D) - beyond system boundary.", "lang": "en"}, {"value": "Gültigkeitsbereich: \nDie Daten wurden von den sieben nach ISO 14001 zertifizierten Fabriken von Ravago Building Solutions, die diese Produkte in Frankreich, Deutschland, Griechenland, Ungarn und Großbritannien herstellen, für das Jahr 2021 zur Verfügung gestellt. \nSystemgrenze: \nTyp der EPD nach EN 15804: \"Cradle to Gate mit Optionen, Module C1-C4 und Modul D\". Die folgenden Module sind deklariert: A1-A3, C, D und zusätzliche Module: A4 + A5. \n\nProduktion - Module A1-A3 Die Produktstufe umfasst: Rohstoffversorgung einschließlich Sekundärmaterialien (A1) Transport zum Hersteller (A2): Der Transport wird für alle Input-Rohstoffe berücksichtigt. Die Herstellung (A3) umfasst die Bereitstellung aller Materialien, Produkte und Energie sowie die Abfallverarbeitung bis hin zum End-of-Waste-Zustand.\nBauphase - Module A4-A5 Die Bauprozessphase umfasst: Transport zur Baustelle (A4) Behandlung des Verpackungsmaterials (A5) End-of-Life-Phase - Module C1-C4 und D Die End-of-Life-Phase umfasst: Manuelle Demontage (lastfrei) (C1) Transport zum EoL (C2) Abfallverarbeitung & Entsorgung (C) mit zwei 100 %-Szenarien (Szenario 1: Verbrennung (C3 und D); Szenario 2: Deponie (C4)) Wiederverwendungs-, Verwertungs- oder Recyclingpotenzial (D) - über die Systemgrenze hinaus.", "lang": "de"}], "other": {"anies": [{"name": "referenceToOriginalEPD", "value": {"shortDescription": {"value": "RAVATHERM™ XPS (X) extruded polystyrene foam insulation with non-halogenated blowing agents.pdf", "defaultValue": "RAVATHERM™ XPS (X) extruded polystyrene foam insulation with non-halogenated blowing agents.pdf", "lstrings": [{"lang": "en", "value": "RAVATHERM™ XPS (X) extruded polystyrene foam insulation with non-halogenated blowing agents.pdf"}]}, "type": "source data set", "uuid": {"uuid": "4082b7a0-1008-4925-b9ec-80ab4e716d88"}, "refObjectId": "4082b7a0-1008-4925-b9ec-80ab4e716d88", "resourceURLs": ["https://oekobaudat.de/OEKOBAU.DAT/resource/sources/4082b7a0-1008-4925-b9ec-80ab4e716d88/RAVATHERM_XPS_X_extruded_polystyrene_foam_insulation_with_non-halogenated_blowing_agents_16709.pdf?version=00.01.000"]}}]}}, "validation": {"review": [{"referenceToNameOfReviewerAndInstitution": [{"shortDescription": [{"value": "Institut Bauen und Umwelt e. V.", "lang": "en"}], "type": "contact data set", "refObjectId": "d111dbec-b024-4be5-86c5-752d6eb2cf95", "uri": "../contacts/d111dbec-b024-4be5-86c5-752d6eb2cf95.xml"}], "type": "Accredited third party review"}]}, "complianceDeclarations": {"compliance": [{"referenceToComplianceSystem": {"shortDescription": [{"value": "DIN EN 15804+A2", "lang": "en"}], "type": "source data set", "refObjectId": "c0016b33-8cf7-415c-ac6e-deba0d21440d", "uri": "../sources/c0016b33-8cf7-415c-ac6e-deba0d21440d.xml"}}, {"referenceToComplianceSystem": {"shortDescription": [{"value": "ISO 14025", "lang": "en"}], "type": "source data set", "refObjectId": "4f2eb655-6e44-4874-a95a-e28f5442cd4d", "uri": "../sources/4f2eb655-6e44-4874-a95a-e28f5442cd4d.xml"}}]}}, "administrativeInformation": {"commissionerAndGoal": {"referenceToCommissioner": [{"shortDescription": [{"value": "RBS Germany GmbH", "lang": "en"}], "type": "contact data set", "refObjectId": "c870f41a-0149-487d-abf3-dc33496a4e4f", "uri": "../contacts/c870f41a-0149-487d-abf3-dc33496a4e4f.xml"}]}, "dataGenerator": {"referenceToPersonOrEntityGeneratingTheDataSet": [{"shortDescription": [{"value": "Sphera Solutions GmbH", "lang": "en"}], "type": "contact data set", "refObjectId": "623edf96-39d1-4e6f-9892-674c7228546b", "uri": "../contacts/623edf96-39d1-4e6f-9892-674c7228546b.xml"}]}, "dataEntryBy": {"timeStamp": 1698710400000, "referenceToDataSetFormat": [{"shortDescription": [{"value": "ILCD Format", "lang": "en"}], "type": "source data set", "refObjectId": "a97a0155-0234-4b87-b4ce-a45da52f2a40", "uri": "../sources/a97a0155-0234-4b87-b4ce-a45da52f2a40.xml"}, {"shortDescription": [{"value": "EPD-Datenformaterweiterungen v1.2", "lang": "de"}, {"value": "EPD Data Format Extensions v1.2", "lang": "en"}], "type": "source data set", "refObjectId": "a29449fd-aa2f-4de8-b5d7-4b06b43c6fde", "uri": "../sources/a29449fd-aa2f-4de8-b5d7-4b06b43c6fde.xml"}]}, "publicationAndOwnership": {"dataSetVersion": "00.03.000", "referenceToRegistrationAuthority": {"shortDescription": [{"value": "Institut Bauen und Umwelt e. V.", "lang": "en"}], "type": "contact data set", "refObjectId": "d111dbec-b024-4be5-86c5-752d6eb2cf95", "uri": "../contacts/d111dbec-b024-4be5-86c5-752d6eb2cf95.xml"}, "registrationNumber": "EPD-RAV-20230375-CBD1-EN", "referenceToOwnershipOfDataSet": {"shortDescription": [{"value": "RBS Germany GmbH", "lang": "en"}], "type": "contact data set", "refObjectId": "c870f41a-0149-487d-abf3-dc33496a4e4f", "uri": "../contacts/c870f41a-0149-487d-abf3-dc33496a4e4f.xml"}, "copyright": true, "licenseType": "Free of charge for all users and uses", "accessRestrictions": [{"value": "None", "lang": "en"}], "other": {"anies": [{"name": "referenceToPublisher", "value": {"shortDescription": [{"value": "Institut Bauen und Umwelt e. V.", "lang": "en"}], "type": "contact data set", "refObjectId": "d111dbec-b024-4be5-86c5-752d6eb2cf95", "uri": "../contacts/d111dbec-b024-4be5-86c5-752d6eb2cf95.xml"}}]}}}, "exchanges": {"exchange": [{"dataSetInternalID": 0, "referenceToFlowDataSet": {"shortDescription": [{"value": "RAVATHERM™ XPS product (RAVATHERM™ XPS product)", "lang": "en"}], "type": "flow data set", "refObjectId": "232de8fe-9b04-777f-f74a-b2ac05b094c2", "uri": "../flows/232de8fe-9b04-777f-f74a-b2ac05b094c2.xml"}, "meanAmount": 1.0, "referencesToDataSource": {}, "referenceFlow": true, "resolvedFlowVersion": "00.03.000", "resultingflowAmount": 1.0, "flowProperties": [{"name": [{"lang": "en", "value": "Volume"}, {"lang": "de", "value": "Volumen"}], "uuid": "93a60a56-a3c8-22da-a746-0800200c9a66", "referenceFlowProperty": true, "meanValue": 1.0, "referenceUnit": "m3", "unitGroupUUID": "cd950537-0a98-4044-9ba7-9f9a68d0a504"}], "materialProperties": [{"name": "gross density", "value": "34.4", "unit": "kg/m^3", "unitDescription": "kilograms per cubic metre"}], "typeOfFlow": "Product flow", "classification": {"classHierarchy": "Dämmstoffe / Extrudiertes Polystyrol (XPS) / XPS weiß", "name": "OEKOBAU.DAT"}}, {"dataSetInternalID": 1, "referenceToFlowDataSet": {"shortDescription": [{"value": "Renewable primary energy as energy carrier (PERE)", "lang": "en"}, {"value": "Erneuerbare Primärenergie als Energieträger (PERE)", "lang": "de"}], "type": "flow data set", "refObjectId": "20f32be5-0398-4288-9b6d-accddd195317", "uri": "../flows/20f32be5-0398-4288-9b6d-accddd195317.xml"}, "exchange direction": "INPUT", "other": {"anies": [{"name": "referenceToUnitGroupDataSet", "value": {"shortDescription": [{"value": "MJ", "lang": "en"}], "type": "unit group data set", "refObjectId": "93a60a57-a3c8-11da-a746-0800200c9a66", "uri": "../unitgroups/93a60a57-a3c8-11da-a746-0800200c9a66.xml"}}, {"value": "98.9632730078787", "module": "A1-A3"}, {"value": "2.28528699648956", "module": "A4"}, {"value": "0.220210009294159", "module": "A5"}, {"value": "0", "module": "C1"}, {"value": "0.212028982971521", "module": "C2"}, {"value": "3.05961677853603", "module": "C3"}, {"value": "2.84150003836493", "module": "C4"}, {"value": "-56.3940708040177", "module": "D", "scenario": "S1"}, {"value": "-2.39425825638457", "module": "D", "scenario": "S2"}]}, "resolvedFlowVersion": "38.00.000", "flowProperties": [], "typeOfFlow": "Other flow", "classification": {"classHierarchy": "Quantities", "name": "GaBiCategories"}}, {"dataSetInternalID": 2, "referenceToFlowDataSet": {"shortDescription": [{"value": "Renewable primary energy resources as material utilization (PERM)", "lang": "en"}, {"value": "Erneuerbare Primärenergie zur stofflichen Nutzung (PERM)", "lang": "de"}], "type": "flow data set", "refObjectId": "fb3ec0de-548d-4508-aea5-00b73bf6f702", "uri": "../flows/fb3ec0de-548d-4508-aea5-00b73bf6f702.xml"}, "exchange direction": "INPUT", "other": {"anies": [{"name": "referenceToUnitGroupDataSet", "value": {"shortDescription": [{"value": "MJ", "lang": "en"}], "type": "unit group data set", "refObjectId": "93a60a57-a3c8-11da-a746-0800200c9a66", "uri": "../unitgroups/93a60a57-a3c8-11da-a746-0800200c9a66.xml"}}, {"value": "0.135", "module": "A1-A3"}, {"value": "0", "module": "A4"}, {"value": "-0.135", "module": "A5"}, {"value": "0", "module": "C1"}, {"value": "0", "module": "C2"}, {"value": "0", "module": "C3"}, {"value": "0", "module": "C4"}, {"value": "0", "module": "D", "scenario": "S1"}, {"value": "0", "module": "D", "scenario": "S2"}]}, "resolvedFlowVersion": "38.00.000", "flowProperties": [], "typeOfFlow": "Other flow", "classification": {"classHierarchy": "Quantities", "name": "GaBiCategories"}}, {"dataSetInternalID": 3, "referenceToFlowDataSet": {"shortDescription": [{"value": "Total use of renewable primary energy resources (PERT)", "lang": "en"}, {"value": "Total erneuerbare Primärenergie (PERT)", "lang": "de"}], "type": "flow data set", "refObjectId": "53f97275-fa8a-4cdd-9024-65936002acd0", "uri": "../flows/53f97275-fa8a-4cdd-9024-65936002acd0.xml"}, "exchange direction": "INPUT", "other": {"anies": [{"name": "referenceToUnitGroupDataSet", "value": {"shortDescription": [{"value": "MJ", "lang": "en"}], "type": "unit group data set", "refObjectId": "93a60a57-a3c8-11da-a746-0800200c9a66", "uri": "../unitgroups/93a60a57-a3c8-11da-a746-0800200c9a66.xml"}}, {"value": "99.0982730078787", "module": "A1-A3"}, {"value": "2.28528699648956", "module": "A4"}, {"value": "0.0852100092941586", "module": "A5"}, {"value": "0", "module": "C1"}, {"value": "0.212028982971521", "module": "C2"}, {"value": "3.05961677853603", "module": "C3"}, {"value": "2.84150003836493", "module": "C4"}, {"value": "-56.3940708040177", "module": "D", "scenario": "S1"}, {"value": "-2.39425825638457", "module": "D", "scenario": "S2"}]}, "resolvedFlowVersion": "38.00.000", "flowProperties": [], "typeOfFlow": "Other flow", "classification": {"classHierarchy": "Quantities / Environmental quantities / EPD EN 15804 / LCI indicators", "name": "GaBiCategories"}}, {"dataSetInternalID": 4, "referenceToFlowDataSet": {"shortDescription": [{"value": "Non renewable primary energy as energy carrier (PENRE)", "lang": "en"}, {"value": "Nicht-erneuerbare Primärenergie als Energieträger (PENRE)", "lang": "de"}], "type": "flow data set", "refObjectId": "ac857178-2b45-46ec-892a-a9a4332f0372", "uri": "../flows/ac857178-2b45-46ec-892a-a9a4332f0372.xml"}, "exchange direction": "INPUT", "other": {"anies": [{"name": "referenceToUnitGroupDataSet", "value": {"shortDescription": [{"value": "MJ", "lang": "en"}], "type": "unit group data set", "refObjectId": "93a60a57-a3c8-11da-a746-0800200c9a66", "uri": "../unitgroups/93a60a57-a3c8-11da-a746-0800200c9a66.xml"}}, {"value": "1483.94870197684", "module": "A1-A3"}, {"value": "40.2955507271646", "module": "A4"}, {"value": "43.2398439327842", "module": "A5"}, {"value": "0", "module": "C1"}, {"value": "3.73862217396864", "module": "C2"}, {"value": "1295.5778615526", "module": "C3"}, {"value": "34.5806178520048", "module": "C4"}, {"value": "-683.484066812037", "module": "D", "scenario": "S1"}, {"value": "-28.9995379919537", "module": "D", "scenario": "S2"}]}, "resolvedFlowVersion": "38.00.000", "flowProperties": [], "typeOfFlow": "Other flow", "classification": {"classHierarchy": "Quantities", "name": "GaBiCategories"}}, {"dataSetInternalID": 5, "referenceToFlowDataSet": {"shortDescription": [{"value": "Non renewable primary energy as material utilization (PENRM)", "lang": "en"}, {"value": "Nicht-erneuerbare Primärenergie zur stofflichen Nutzung (PENRM)", "lang": "de"}], "type": "flow data set", "refObjectId": "1421caa0-679d-4bf4-b282-0eb850ccae27", "uri": "../flows/1421caa0-679d-4bf4-b282-0eb850ccae27.xml"}, "exchange direction": "INPUT", "other": {"anies": [{"name": "referenceToUnitGroupDataSet", "value": {"shortDescription": [{"value": "MJ", "lang": "en"}], "type": "unit group data set", "refObjectId": "93a60a57-a3c8-11da-a746-0800200c9a66", "uri": "../unitgroups/93a60a57-a3c8-11da-a746-0800200c9a66.xml"}}, {"value": "1325.68", "module": "A1-A3"}, {"value": "0", "module": "A4"}, {"value": "-42.88", "module": "A5"}, {"value": "0", "module": "C1"}, {"value": "0", "module": "C2"}, {"value": "-1282.8", "module": "C3"}, {"value": "0", "module": "C4"}, {"value": "0", "module": "D", "scenario": "S1"}, {"value": "0", "module": "D", "scenario": "S2"}]}, "resolvedFlowVersion": "38.00.000", "flowProperties": [], "typeOfFlow": "Other flow", "classification": {"classHierarchy": "Quantities", "name": "GaBiCategories"}}, {"dataSetInternalID": 6, "referenceToFlowDataSet": {"shortDescription": [{"value": "Total use of non renewable primary energy resources (PENRT)", "lang": "en"}, {"value": "Total nicht erneuerbare Primärenergie (PENRT)", "lang": "de"}], "type": "flow data set", "refObjectId": "06159210-646b-4c8d-8583-da9b3b95a6c1", "uri": "../flows/06159210-646b-4c8d-8583-da9b3b95a6c1.xml"}, "exchange direction": "INPUT", "other": {"anies": [{"name": "referenceToUnitGroupDataSet", "value": {"shortDescription": [{"value": "MJ", "lang": "en"}], "type": "unit group data set", "refObjectId": "93a60a57-a3c8-11da-a746-0800200c9a66", "uri": "../unitgroups/93a60a57-a3c8-11da-a746-0800200c9a66.xml"}}, {"value": "2809.62870197684", "module": "A1-A3"}, {"value": "40.2955507271646", "module": "A4"}, {"value": "0.359843932784174", "module": "A5"}, {"value": "0", "module": "C1"}, {"value": "3.73862217396864", "module": "C2"}, {"value": "12.7778615526016", "module": "C3"}, {"value": "34.5806178520048", "module": "C4"}, {"value": "-683.484066812043", "module": "D", "scenario": "S1"}, {"value": "-28.9995379919539", "module": "D", "scenario": "S2"}]}, "resolvedFlowVersion": "38.00.000", "flowProperties": [], "typeOfFlow": "Other flow", "classification": {"classHierarchy": "Quantities / Environmental quantities / EPD EN 15804 / LCI indicators", "name": "GaBiCategories"}}, {"dataSetInternalID": 7, "referenceToFlowDataSet": {"shortDescription": [{"value": "Use of secondary material (SM)", "lang": "en"}, {"value": "Einsatz von Sekundärstoffen (SM)", "lang": "de"}], "type": "flow data set", "refObjectId": "c6a1f35f-2d09-4f54-8dfb-97e502e1ce92", "uri": "../flows/c6a1f35f-2d09-4f54-8dfb-97e502e1ce92.xml"}, "exchange direction": "INPUT", "other": {"anies": [{"name": "referenceToUnitGroupDataSet", "value": {"shortDescription": [{"value": "kg", "lang": "en"}], "type": "unit group data set", "refObjectId": "ad38d542-3fe9-439d-9b95-2f5f7752acaf", "uri": "../unitgroups/ad38d542-3fe9-439d-9b95-2f5f7752acaf.xml"}}, {"value": "9.48", "module": "A1-A3"}, {"value": "0", "module": "A4"}, {"value": "0", "module": "A5"}, {"value": "0", "module": "C1"}, {"value": "0", "module": "C2"}, {"value": "0", "module": "C3"}, {"value": "0", "module": "C4"}, {"value": "0", "module": "D", "scenario": "S1"}, {"value": "0", "module": "D", "scenario": "S2"}]}, "resolvedFlowVersion": "38.00.000", "flowProperties": [], "typeOfFlow": "Other flow", "classification": {"classHierarchy": "Quantities / Environmental quantities / EPD EN 15804 / LCI indicators", "name": "GaBiCategories"}}, {"dataSetInternalID": 8, "referenceToFlowDataSet": {"shortDescription": [{"value": "Use of renewable secondary fuels (RSF)", "lang": "en"}, {"value": "Erneuerbare Sekundärbrennstoffe (RSF)", "lang": "de"}], "type": "flow data set", "refObjectId": "64333088-a55f-4aa2-9a31-c10b07816787", "uri": "../flows/64333088-a55f-4aa2-9a31-c10b07816787.xml"}, "exchange direction": "INPUT", "other": {"anies": [{"name": "referenceToUnitGroupDataSet", "value": {"shortDescription": [{"value": "MJ", "lang": "en"}], "type": "unit group data set", "refObjectId": "93a60a57-a3c8-11da-a746-0800200c9a66", "uri": "../unitgroups/93a60a57-a3c8-11da-a746-0800200c9a66.xml"}}, {"value": "0", "module": "A1-A3"}, {"value": "0", "module": "A4"}, {"value": "0", "module": "A5"}, {"value": "0", "module": "C1"}, {"value": "0", "module": "C2"}, {"value": "0", "module": "C3"}, {"value": "0", "module": "C4"}, {"value": "0", "module": "D", "scenario": "S1"}, {"value": "0", "module": "D", "scenario": "S2"}]}, "resolvedFlowVersion": "38.00.000", "flowProperties": [], "typeOfFlow": "Other flow", "classification": {"classHierarchy": "Quantities / Environmental quantities / EPD EN 15804 / LCI indicators", "name": "GaBiCategories"}}, {"dataSetInternalID": 9, "referenceToFlowDataSet": {"shortDescription": [{"value": "Use of non renewable secondary fuels (NRSF)", "lang": "en"}, {"value": "Nicht erneuerbare Sekundärbrennstoffe (NRSF)", "lang": "de"}], "type": "flow data set", "refObjectId": "89def144-d39a-4287-b86f-efde453ddcb2", "uri": "../flows/89def144-d39a-4287-b86f-efde453ddcb2.xml"}, "exchange direction": "INPUT", "other": {"anies": [{"name": "referenceToUnitGroupDataSet", "value": {"shortDescription": [{"value": "MJ", "lang": "en"}], "type": "unit group data set", "refObjectId": "93a60a57-a3c8-11da-a746-0800200c9a66", "uri": "../unitgroups/93a60a57-a3c8-11da-a746-0800200c9a66.xml"}}, {"value": "0", "module": "A1-A3"}, {"value": "0", "module": "A4"}, {"value": "0", "module": "A5"}, {"value": "0", "module": "C1"}, {"value": "0", "module": "C2"}, {"value": "0", "module": "C3"}, {"value": "0", "module": "C4"}, {"value": "0", "module": "D", "scenario": "S1"}, {"value": "0", "module": "D", "scenario": "S2"}]}, "resolvedFlowVersion": "38.00.000", "flowProperties": [], "typeOfFlow": "Other flow", "classification": {"classHierarchy": "Quantities / Environmental quantities / EPD EN 15804 / LCI indicators", "name": "GaBiCategories"}}, {"dataSetInternalID": 10, "referenceToFlowDataSet": {"shortDescription": [{"value": "Use of net fresh water (FW)", "lang": "en"}, {"value": "Einsatz von Süßwasserressourcen (FW)", "lang": "de"}], "type": "flow data set", "refObjectId": "3cf952c8-f3a4-461d-8c96-96456ca62246", "uri": "../flows/3cf952c8-f3a4-461d-8c96-96456ca62246.xml"}, "exchange direction": "INPUT", "other": {"anies": [{"name": "referenceToUnitGroupDataSet", "value": {"shortDescription": [{"value": "m^3", "lang": "en"}], "type": "unit group data set", "refObjectId": "cd950537-0a98-4044-9ba7-9f9a68d0a504", "uri": "../unitgroups/cd950537-0a98-4044-9ba7-9f9a68d0a504.xml"}}, {"value": "0.46802221372653", "module": "A1-A3"}, {"value": "0.00258454317022666", "module": "A4"}, {"value": "0.00650413751145662", "module": "A5"}, {"value": "0", "module": "C1"}, {"value": "0.000239793978030305", "module": "C2"}, {"value": "0.220229101938387", "module": "C3"}, {"value": "0.000447421378301893", "module": "C4"}, {"value": "-0.0860202463425104", "module": "D", "scenario": "S1"}, {"value": "-0.00365202462701258", "module": "D", "scenario": "S2"}]}, "resolvedFlowVersion": "38.00.000", "flowProperties": [], "typeOfFlow": "Other flow", "classification": {"classHierarchy": "Quantities / Environmental quantities / EPD EN 15804 / LCI indicators", "name": "GaBiCategories"}}, {"dataSetInternalID": 11, "referenceToFlowDataSet": {"shortDescription": [{"value": "Hazardous waste disposed (HWD)", "lang": "en"}, {"value": "Gefährlicher Abfall zur Deponie (HWD)", "lang": "de"}], "type": "flow data set", "refObjectId": "430f9e0f-59b2-46a0-8e0d-55e0e84948fc", "uri": "../flows/430f9e0f-59b2-46a0-8e0d-55e0e84948fc.xml"}, "exchange direction": "OUTPUT", "other": {"anies": [{"name": "referenceToUnitGroupDataSet", "value": {"shortDescription": [{"value": "kg", "lang": "en"}], "type": "unit group data set", "refObjectId": "ad38d542-3fe9-439d-9b95-2f5f7752acaf", "uri": "../unitgroups/ad38d542-3fe9-439d-9b95-2f5f7752acaf.xml"}}, {"value": "1.52142171187928E-07", "module": "A1-A3"}, {"value": "1.92965706689185E-10", "module": "A4"}, {"value": "3.38386958259435E-11", "module": "A5"}, {"value": "0", "module": "C1"}, {"value": "1.79033629476462E-11", "module": "C2"}, {"value": "1.19908170514494E-09", "module": "C3"}, {"value": "5.33161865973199E-09", "module": "C4"}, {"value": "-8.22512785666371E-08", "module": "D", "scenario": "S1"}, {"value": "-3.48864490759554E-09", "module": "D", "scenario": "S2"}]}, "resolvedFlowVersion": "38.00.000", "flowProperties": [], "typeOfFlow": "Other flow", "classification": {"classHierarchy": "Quantities / Environmental quantities / EPD EN 15804 / LCI indicators", "name": "GaBiCategories"}}, {"dataSetInternalID": 12, "referenceToFlowDataSet": {"shortDescription": [{"value": "Non hazardous waste disposed (NHWD)", "lang": "en"}, {"value": "Entsorgter nicht gefährlicher Abfall (NHWD)", "lang": "de"}], "type": "flow data set", "refObjectId": "b29ef66b-e286-4afa-949f-62f1a7b4d7fa", "uri": "../flows/b29ef66b-e286-4afa-949f-62f1a7b4d7fa.xml"}, "exchange direction": "OUTPUT", "other": {"anies": [{"name": "referenceToUnitGroupDataSet", "value": {"shortDescription": [{"value": "kg", "lang": "en"}], "type": "unit group data set", "refObjectId": "ad38d542-3fe9-439d-9b95-2f5f7752acaf", "uri": "../unitgroups/ad38d542-3fe9-439d-9b95-2f5f7752acaf.xml"}}, {"value": "0.761381225904867", "module": "A1-A3"}, {"value": "0.00577493391600435", "module": "A4"}, {"value": "0.0141554056517348", "module": "A5"}, {"value": "0", "module": "C1"}, {"value": "0.00053579850881707", "module": "C2"}, {"value": "0.661770992784024", "module": "C3"}, {"value": "34.2332203205117", "module": "C4"}, {"value": "-0.161118509751855", "module": "D", "scenario": "S1"}, {"value": "-0.00683552739916278", "module": "D", "scenario": "S2"}]}, "resolvedFlowVersion": "38.00.000", "flowProperties": [], "typeOfFlow": "Other flow", "classification": {"classHierarchy": "Quantities / Environmental quantities / EPD EN 15804 / LCI indicators", "name": "GaBiCategories"}}, {"dataSetInternalID": 13, "referenceToFlowDataSet": {"shortDescription": [{"value": "Radioactive waste disposed (RWD)", "lang": "en"}, {"value": "Entsorgter radioaktiver Abfall (RWD)", "lang": "de"}], "type": "flow data set", "refObjectId": "3449546e-52ad-4b39-b809-9fb77cea8ff6", "uri": "../flows/3449546e-52ad-4b39-b809-9fb77cea8ff6.xml"}, "exchange direction": "OUTPUT", "other": {"anies": [{"name": "referenceToUnitGroupDataSet", "value": {"shortDescription": [{"value": "kg", "lang": "en"}], "type": "unit group data set", "refObjectId": "ad38d542-3fe9-439d-9b95-2f5f7752acaf", "uri": "../unitgroups/ad38d542-3fe9-439d-9b95-2f5f7752acaf.xml"}}, {"value": "0.055065906307094", "module": "A1-A3"}, {"value": "4.96310134591595E-05", "module": "A4"}, {"value": "2.17411906181131E-05", "module": "A5"}, {"value": "0", "module": "C1"}, {"value": "4.60476663270575E-06", "module": "C2"}, {"value": "0.000770163565317333", "module": "C3"}, {"value": "0.000424700292809739", "module": "C4"}, {"value": "-0.0637526793330835", "module": "D", "scenario": "S1"}, {"value": "-0.00270674307473327", "module": "D", "scenario": "S2"}]}, "resolvedFlowVersion": "38.00.000", "flowProperties": [], "typeOfFlow": "Other flow", "classification": {"classHierarchy": "Quantities / Environmental quantities / EPD EN 15804 / LCI indicators", "name": "GaBiCategories"}}, {"dataSetInternalID": 14, "referenceToFlowDataSet": {"shortDescription": [{"value": "Components for re-use (CRU)", "lang": "en"}, {"value": "Komponenten für die Wiederverwendung (CRU)", "lang": "de"}], "type": "flow data set", "refObjectId": "a2b32f97-3fc7-4af2-b209-525bc6426f33", "uri": "../flows/a2b32f97-3fc7-4af2-b209-525bc6426f33.xml"}, "exchange direction": "OUTPUT", "other": {"anies": [{"name": "referenceToUnitGroupDataSet", "value": {"shortDescription": [{"value": "kg", "lang": "en"}], "type": "unit group data set", "refObjectId": "ad38d542-3fe9-439d-9b95-2f5f7752acaf", "uri": "../unitgroups/ad38d542-3fe9-439d-9b95-2f5f7752acaf.xml"}}, {"value": "0", "module": "A1-A3"}, {"value": "0", "module": "A4"}, {"value": "0", "module": "A5"}, {"value": "0", "module": "C1"}, {"value": "0", "module": "C2"}, {"value": "0", "module": "C3"}, {"value": "0", "module": "C4"}, {"value": "0", "module": "D", "scenario": "S1"}, {"value": "0", "module": "D", "scenario": "S2"}]}, "resolvedFlowVersion": "38.00.000", "flowProperties": [], "typeOfFlow": "Other flow", "classification": {"classHierarchy": "Quantities / Environmental quantities / EPD EN 15804 / LCI indicators", "name": "GaBiCategories"}}, {"dataSetInternalID": 15, "referenceToFlowDataSet": {"shortDescription": [{"value": "Materials for recycling (MFR)", "lang": "en"}, {"value": "Stoffe zum Recycling (MFR)", "lang": "de"}], "type": "flow data set", "refObjectId": "d7fe48a5-4103-49c8-9aae-b0b5dfdbd6ae", "uri": "../flows/d7fe48a5-4103-49c8-9aae-b0b5dfdbd6ae.xml"}, "exchange direction": "OUTPUT", "other": {"anies": [{"name": "referenceToUnitGroupDataSet", "value": {"shortDescription": [{"value": "kg", "lang": "en"}], "type": "unit group data set", "refObjectId": "ad38d542-3fe9-439d-9b95-2f5f7752acaf", "uri": "../unitgroups/ad38d542-3fe9-439d-9b95-2f5f7752acaf.xml"}}, {"value": "0", "module": "A1-A3"}, {"value": "0", "module": "A4"}, {"value": "0", "module": "A5"}, {"value": "0", "module": "C1"}, {"value": "0", "module": "C2"}, {"value": "0", "module": "C3"}, {"value": "0", "module": "C4"}, {"value": "0", "module": "D", "scenario": "S1"}, {"value": "0", "module": "D", "scenario": "S2"}]}, "resolvedFlowVersion": "38.00.000", "flowProperties": [], "typeOfFlow": "Other flow", "classification": {"classHierarchy": "Quantities / Environmental quantities / EPD EN 15804 / LCI indicators", "name": "GaBiCategories"}}, {"dataSetInternalID": 16, "referenceToFlowDataSet": {"shortDescription": [{"value": "Materials for energy recovery (MER)", "lang": "en"}, {"value": "Stoffe für die Energierückgewinnung (MER)", "lang": "de"}], "type": "flow data set", "refObjectId": "59a9181c-3aaf-46ee-8b13-2b3723b6e447", "uri": "../flows/59a9181c-3aaf-46ee-8b13-2b3723b6e447.xml"}, "exchange direction": "OUTPUT", "other": {"anies": [{"name": "referenceToUnitGroupDataSet", "value": {"shortDescription": [{"value": "kg", "lang": "en"}], "type": "unit group data set", "refObjectId": "ad38d542-3fe9-439d-9b95-2f5f7752acaf", "uri": "../unitgroups/ad38d542-3fe9-439d-9b95-2f5f7752acaf.xml"}}, {"value": "0", "module": "A1-A3"}, {"value": "0", "module": "A4"}, {"value": "0", "module": "A5"}, {"value": "0", "module": "C1"}, {"value": "0", "module": "C2"}, {"value": "0", "module": "C3"}, {"value": "0", "module": "C4"}, {"value": "0", "module": "D", "scenario": "S1"}, {"value": "0", "module": "D", "scenario": "S2"}]}, "resolvedFlowVersion": "38.00.000", "flowProperties": [], "typeOfFlow": "Other flow", "classification": {"classHierarchy": "Quantities / Environmental quantities / EPD EN 15804 / LCI indicators", "name": "GaBiCategories"}}, {"dataSetInternalID": 17, "referenceToFlowDataSet": {"shortDescription": [{"value": "Exported electrical energy (EEE)", "lang": "en"}, {"value": "Exportierte elektrische Energie (EEE)", "lang": "de"}], "type": "flow data set", "refObjectId": "4da0c987-2b76-40d6-9e9e-82a017aaaf29", "uri": "../flows/4da0c987-2b76-40d6-9e9e-82a017aaaf29.xml"}, "exchange direction": "OUTPUT", "other": {"anies": [{"name": "referenceToUnitGroupDataSet", "value": {"shortDescription": [{"value": "MJ", "lang": "en"}], "type": "unit group data set", "refObjectId": "93a60a57-a3c8-11da-a746-0800200c9a66", "uri": "../unitgroups/93a60a57-a3c8-11da-a746-0800200c9a66.xml"}}, {"value": "0.363795163131031", "module": "A1-A3"}, {"value": "0", "module": "A4"}, {"value": "6.32768195497157", "module": "A5"}, {"value": "0", "module": "C1"}, {"value": "0", "module": "C2"}, {"value": "208.393995946892", "module": "C3"}, {"value": "0", "module": "C4"}, {"value": "0", "module": "D", "scenario": "S1"}, {"value": "0", "module": "D", "scenario": "S2"}]}, "resolvedFlowVersion": "38.00.000", "flowProperties": [], "typeOfFlow": "Other flow", "classification": {"classHierarchy": "Quantities / Environmental quantities / EPD EN 15804 / LCI indicators", "name": "GaBiCategories"}}, {"dataSetInternalID": 18, "referenceToFlowDataSet": {"shortDescription": [{"value": "Exported thermal energy (EET)", "lang": "en"}, {"value": "Exportierte thermische Energie (EET)", "lang": "de"}], "type": "flow data set", "refObjectId": "98daf38a-7a79-46d3-9a37-2b7bd0955810", "uri": "../flows/98daf38a-7a79-46d3-9a37-2b7bd0955810.xml"}, "exchange direction": "OUTPUT", "other": {"anies": [{"name": "referenceToUnitGroupDataSet", "value": {"shortDescription": [{"value": "MJ", "lang": "en"}], "type": "unit group data set", "refObjectId": "93a60a57-a3c8-11da-a746-0800200c9a66", "uri": "../unitgroups/93a60a57-a3c8-11da-a746-0800200c9a66.xml"}}, {"value": "0.648405014415144", "module": "A1-A3"}, {"value": "0", "module": "A4"}, {"value": "11.2593371547996", "module": "A5"}, {"value": "0", "module": "C1"}, {"value": "0", "module": "C2"}, {"value": "371.428005757475", "module": "C3"}, {"value": "0", "module": "C4"}, {"value": "0", "module": "D", "scenario": "S1"}, {"value": "0", "module": "D", "scenario": "S2"}]}, "resolvedFlowVersion": "38.00.000", "flowProperties": [], "typeOfFlow": "Other flow", "classification": {"classHierarchy": "Quantities / Environmental quantities / EPD EN 15804 / LCI indicators", "name": "GaBiCategories"}}]}, "LCIAResults": {"LCIAResult": [{"referenceToLCIAMethodDataSet": {"shortDescription": [{"value": "Global Warming Potential total (GWP-total)", "lang": "en"}, {"value": "Globales Erwärmungspotenzial total (GWP-total)", "lang": "de"}], "type": "LCIA method data set", "refObjectId": "6a37f984-a4b3-458a-a20a-64418c145fa2", "uri": "../lciamethods/6a37f984-a4b3-458a-a20a-64418c145fa2.xml"}, "other": {"anies": [{"name": "referenceToUnitGroupDataSet", "value": {"shortDescription": [{"value": "kg CO_(2) eq", "lang": "en"}], "type": "unit group data set", "refObjectId": "1ebf3012-d0db-4de2-aefd-ef30cedb0be1", "uri": "../unitgroups/1ebf3012-d0db-4de2-aefd-ef30cedb0be1.xml"}}, {"value": "93.8393524649814", "module": "A1-A3"}, {"value": "3.01181964821407", "module": "A4"}, {"value": "3.10929220338491", "module": "A5"}, {"value": "0", "module": "C1"}, {"value": "0.279436700022982", "module": "C2"}, {"value": "115.118344637212", "module": "C3"}, {"value": "2.44226815433566", "module": "C4"}, {"value": "-36.840536734704", "module": "D", "scenario": "S1"}, {"value": "-1.56294256020943", "module": "D", "scenario": "S2"}]}}, {"referenceToLCIAMethodDataSet": {"shortDescription": [{"value": "Global Warming Potential fossil fuels (GWP-fossil)", "lang": "en"}, {"value": "Globales Erwärmungspotenzial fossil (GWP-fossil)", "lang": "de"}], "type": "LCIA method data set", "refObjectId": "5f635281-343e-44fb-83df-1971b155e6b6", "uri": "../lciamethods/5f635281-343e-44fb-83df-1971b155e6b6.xml"}, "other": {"anies": [{"name": "referenceToUnitGroupDataSet", "value": {"shortDescription": [{"value": "kg CO_(2) eq", "lang": "en"}], "type": "unit group data set", "refObjectId": "1ebf3012-d0db-4de2-aefd-ef30cedb0be1", "uri": "../unitgroups/1ebf3012-d0db-4de2-aefd-ef30cedb0be1.xml"}}, {"value": "93.7795532567059", "module": "A1-A3"}, {"value": "2.98236981301655", "module": "A4"}, {"value": "3.10111717202973", "module": "A5"}, {"value": "0", "module": "C1"}, {"value": "0.276704343598953", "module": "C2"}, {"value": "115.11477443848", "module": "C3"}, {"value": "2.43594085456207", "module": "C4"}, {"value": "-36.7946896538555", "module": "D", "scenario": "S1"}, {"value": "-1.56099819906286", "module": "D", "scenario": "S2"}]}}, {"referenceToLCIAMethodDataSet": {"shortDescription": [{"value": "Global Warming Potential biogenic (GWP-biogenic)", "lang": "en"}, {"value": "Globales Erwärmungspotenzial biogen (GWP-biogenic)", "lang": "de"}], "type": "LCIA method data set", "refObjectId": "2356e1ab-0185-4db5-86e5-16de51c7485c", "uri": "../lciamethods/2356e1ab-0185-4db5-86e5-16de51c7485c.xml"}, "other": {"anies": [{"name": "referenceToUnitGroupDataSet", "value": {"shortDescription": [{"value": "kg CO_(2) eq", "lang": "en"}], "type": "unit group data set", "refObjectId": "1ebf3012-d0db-4de2-aefd-ef30cedb0be1", "uri": "../unitgroups/1ebf3012-d0db-4de2-aefd-ef30cedb0be1.xml"}}, {"value": "0.0313355950816808", "module": "A1-A3"}, {"value": "0.0126787658249383", "module": "A4"}, {"value": "0.0081716111100404", "module": "A5"}, {"value": "0", "module": "C1"}, {"value": "0.00117633620080332", "module": "C2"}, {"value": "0.00343513767246963", "module": "C3"}, {"value": "0.00514139046054249", "module": "C4"}, {"value": "-0.0442418189354167", "module": "D", "scenario": "S1"}, {"value": "-0.00187623416585539", "module": "D", "scenario": "S2"}]}}, {"referenceToLCIAMethodDataSet": {"shortDescription": [{"value": "Global Warming Potential luluc (GWP-luluc)", "lang": "en"}, {"value": "Globales Erwärmungspotenzial luluc (GWP-luluc)", "lang": "de"}], "type": "LCIA method data set", "refObjectId": "4331bbdb-978a-490d-8707-eeb047f01a55", "uri": "../lciamethods/4331bbdb-978a-490d-8707-eeb047f01a55.xml"}, "other": {"anies": [{"name": "referenceToUnitGroupDataSet", "value": {"shortDescription": [{"value": "kg CO_(2) eq", "lang": "en"}], "type": "unit group data set", "refObjectId": "1ebf3012-d0db-4de2-aefd-ef30cedb0be1", "uri": "../unitgroups/1ebf3012-d0db-4de2-aefd-ef30cedb0be1.xml"}}, {"value": "0.0284636131938685", "module": "A1-A3"}, {"value": "0.0167710693725819", "module": "A4"}, {"value": "3.42024513329981E-06", "module": "A5"}, {"value": "0", "module": "C1"}, {"value": "0.00155602022322609", "module": "C2"}, {"value": "0.000135061059227298", "module": "C3"}, {"value": "0.00118590931304585", "module": "C4"}, {"value": "-0.00160526191301158", "module": "D", "scenario": "S1"}, {"value": "-6.8126980713361E-05", "module": "D", "scenario": "S2"}]}}, {"referenceToLCIAMethodDataSet": {"shortDescription": [{"value": "Depletion potential of the stratospheric ozone layer (ODP)", "lang": "en"}, {"value": "Abbau Potential der stratosphärischen Ozonschicht (ODP)", "lang": "de"}], "type": "LCIA method data set", "refObjectId": "b5c629d6-def3-11e6-bf01-fe55135034f3", "uri": "../lciamethods/b5c629d6-def3-11e6-bf01-fe55135034f3.xml"}, "other": {"anies": [{"name": "referenceToUnitGroupDataSet", "value": {"shortDescription": [{"value": "kg CFC11 eq", "lang": "en"}], "type": "unit group data set", "refObjectId": "d9e957c9-7309-4474-bf3a-7777df6c4e5b", "uri": "../unitgroups/d9e957c9-7309-4474-bf3a-7777df6c4e5b.xml"}}, {"value": "1.93870407347766E-10", "module": "A1-A3"}, {"value": "1.80222971663649E-13", "module": "A4"}, {"value": "1.33254288058364E-13", "module": "A5"}, {"value": "0", "module": "C1"}, {"value": "1.67210916828596E-14", "module": "C2"}, {"value": "4.81815652491889E-12", "module": "C3"}, {"value": "3.27195117189263E-12", "module": "C4"}, {"value": "-1.78984931876918E-10", "module": "D", "scenario": "S1"}, {"value": "-7.5991311580089E-12", "module": "D", "scenario": "S2"}]}}, {"referenceToLCIAMethodDataSet": {"shortDescription": [{"value": "Acidification potential of land and water (AP)", "lang": "en"}, {"value": "Versauerungspotenzial von Boden und Wasser (AP)", "lang": "de"}], "type": "LCIA method data set", "refObjectId": "b5c611c6-def3-11e6-bf01-fe55135034f3", "uri": "../lciamethods/b5c611c6-def3-11e6-bf01-fe55135034f3.xml"}, "other": {"anies": [{"name": "referenceToUnitGroupDataSet", "value": {"shortDescription": [{"value": "mol H^(+) eq", "lang": "en"}], "type": "unit group data set", "refObjectId": "42e089ac-92bf-4bf2-8ca1-5fc40d18f2ed", "uri": "../unitgroups/42e089ac-92bf-4bf2-8ca1-5fc40d18f2ed.xml"}}, {"value": "0.146505480306674", "module": "A1-A3"}, {"value": "0.0029699486702496", "module": "A4"}, {"value": "0.000299450372326251", "module": "A5"}, {"value": "0", "module": "C1"}, {"value": "0.000275551909671719", "module": "C2"}, {"value": "0.0101276686166573", "module": "C3"}, {"value": "0.00721952252583448", "module": "C4"}, {"value": "-0.0370907681574595", "module": "D", "scenario": "S1"}, {"value": "-0.0015740898591601", "module": "D", "scenario": "S2"}]}}, {"referenceToLCIAMethodDataSet": {"shortDescription": [{"value": "Eutrophication potential aquatic freshwater (EP-freshwater)", "lang": "en"}, {"value": "Eutrophierungspotenzial Süßwasser (EP-freshwater)", "lang": "de"}], "type": "LCIA method data set", "refObjectId": "b53ec18f-7377-4ad3-86eb-cc3f4f276b2b", "uri": "../lciamethods/b53ec18f-7377-4ad3-86eb-cc3f4f276b2b.xml"}, "other": {"anies": [{"name": "referenceToUnitGroupDataSet", "value": {"shortDescription": [{"value": "kg P eq", "lang": "en"}], "type": "unit group data set", "refObjectId": "0429039d-a61d-4590-ba67-aa4a20a810a1", "uri": "../unitgroups/0429039d-a61d-4590-ba67-aa4a20a810a1.xml"}}, {"value": "0.00014979212540847", "module": "A1-A3"}, {"value": "8.97913611918179E-06", "module": "A4"}, {"value": "3.11067923438212E-08", "module": "A5"}, {"value": "0", "module": "C1"}, {"value": "8.33084466956432E-07", "module": "C2"}, {"value": "1.12738022875191E-06", "module": "C3"}, {"value": "0.000454719408377751", "module": "C4"}, {"value": "-9.2055164405161E-06", "module": "D", "scenario": "S1"}, {"value": "-3.90768662994596E-07", "module": "D", "scenario": "S2"}]}}, {"referenceToLCIAMethodDataSet": {"shortDescription": [{"value": "Eutrophication potential aquatic marine (EP-marine)", "lang": "en"}, {"value": "Eutrophierungspotenzial Salzwasser (EP-marine)", "lang": "de"}], "type": "LCIA method data set", "refObjectId": "b5c619fa-def3-11e6-bf01-fe55135034f3", "uri": "../lciamethods/b5c619fa-def3-11e6-bf01-fe55135034f3.xml"}, "other": {"anies": [{"name": "referenceToUnitGroupDataSet", "value": {"shortDescription": [{"value": "kg N eq", "lang": "en"}], "type": "unit group data set", "refObjectId": "d05bb823-ecdf-4686-8c40-bf1d9257859f", "uri": "../unitgroups/d05bb823-ecdf-4686-8c40-bf1d9257859f.xml"}}, {"value": "0.0381684522402776", "module": "A1-A3"}, {"value": "0.000938151280543046", "module": "A4"}, {"value": "6.36682143544031E-05", "module": "A5"}, {"value": "0", "module": "C1"}, {"value": "8.70416985667564E-05", "module": "C2"}, {"value": "0.00222082566060774", "module": "C3"}, {"value": "0.00159722457950303", "module": "C4"}, {"value": "-0.0117637308619133", "module": "D", "scenario": "S1"}, {"value": "-0.000499165114046151", "module": "D", "scenario": "S2"}]}}, {"referenceToLCIAMethodDataSet": {"shortDescription": [{"value": "Eutrophication potential terrestrial (EP-terrestrial)", "lang": "en"}, {"value": "Eutrophierungspotenzial Land (EP-terrestrial)", "lang": "de"}], "type": "LCIA method data set", "refObjectId": "b5c614d2-def3-11e6-bf01-fe55135034f3", "uri": "../lciamethods/b5c614d2-def3-11e6-bf01-fe55135034f3.xml"}, "other": {"anies": [{"name": "referenceToUnitGroupDataSet", "value": {"shortDescription": [{"value": "mol N eq", "lang": "en"}], "type": "unit group data set", "refObjectId": "71b4d617-0ec9-4d3f-b65e-e438940c2401", "uri": "../unitgroups/71b4d617-0ec9-4d3f-b65e-e438940c2401.xml"}}, {"value": "0.418277709321476", "module": "A1-A3"}, {"value": "0.0113043347834631", "module": "A4"}, {"value": "0.00140364946637349", "module": "A5"}, {"value": "0", "module": "C1"}, {"value": "0.00104881645543386", "module": "C2"}, {"value": "0.0475196391156065", "module": "C3"}, {"value": "0.0175177306254394", "module": "C4"}, {"value": "-0.127547078891781", "module": "D", "scenario": "S1"}, {"value": "-0.00541207602998339", "module": "D", "scenario": "S2"}]}}, {"referenceToLCIAMethodDataSet": {"shortDescription": [{"value": "Formation potential of tropospheric ozone photochemical oxidants (POCP)", "lang": "en"}, {"value": "Bildungspotential für troposphärisches Ozon (POCP)", "lang": "de"}], "type": "LCIA method data set", "refObjectId": "b5c610fe-def3-11e6-bf01-fe55135034f3", "uri": "../lciamethods/b5c610fe-def3-11e6-bf01-fe55135034f3.xml"}, "other": {"anies": [{"name": "referenceToUnitGroupDataSet", "value": {"shortDescription": [{"value": "kg NMVOC eq", "lang": "en"}], "type": "unit group data set", "refObjectId": "d27c25f8-fbc1-44c6-b47b-4adbae4199c6", "uri": "../unitgroups/d27c25f8-fbc1-44c6-b47b-4adbae4199c6.xml"}}, {"value": "0.227781019921483", "module": "A1-A3"}, {"value": "0.00257255298570496", "module": "A4"}, {"value": "0.000188775422499962", "module": "A5"}, {"value": "0", "module": "C1"}, {"value": "0.000238681528419516", "module": "C2"}, {"value": "0.00654404117176617", "module": "C3"}, {"value": "0.00513823495393334", "module": "C4"}, {"value": "-0.0338641900620717", "module": "D", "scenario": "S1"}, {"value": "-0.00143691887448776", "module": "D", "scenario": "S2"}]}}, {"referenceToLCIAMethodDataSet": {"shortDescription": [{"value": "Abiotic depletion potential for non fossil resources (ADPE)", "lang": "en"}, {"value": "Potenzial für den abiotischen Abbau nicht fossiler Ressourcen (ADPE)", "lang": "de"}], "type": "LCIA method data set", "refObjectId": "b2ad6494-c78d-11e6-9d9d-cec0c932ce01", "uri": "../lciamethods/b2ad6494-c78d-11e6-9d9d-cec0c932ce01.xml"}, "other": {"anies": [{"name": "referenceToUnitGroupDataSet", "value": {"shortDescription": [{"value": "kg Sb eq", "lang": "en"}], "type": "unit group data set", "refObjectId": "54ccd2d9-a32a-4fc2-923d-f2c8c93e89d4", "uri": "../unitgroups/54ccd2d9-a32a-4fc2-923d-f2c8c93e89d4.xml"}}, {"value": "1.46721045626982E-05", "module": "A1-A3"}, {"value": "2.5147125788758E-07", "module": "A4"}, {"value": "3.22562849777153E-09", "module": "A5"}, {"value": "0", "module": "C1"}, {"value": "2.33315094070795E-08", "module": "C2"}, {"value": "1.16557096129016E-07", "module": "C3"}, {"value": "1.68929949865787E-07", "module": "C4"}, {"value": "-3.02890938288204E-06", "module": "D", "scenario": "S1"}, {"value": "-1.28542308076121E-07", "module": "D", "scenario": "S2"}]}}, {"referenceToLCIAMethodDataSet": {"shortDescription": [{"value": "Abiotic depletion potential for fossil resources (ADPF)", "lang": "en"}, {"value": "Potenzial für den abiotischen Abbau fossiler Brennstoffe (ADPF)", "lang": "de"}], "type": "LCIA method data set", "refObjectId": "b2ad6110-c78d-11e6-9d9d-cec0c932ce01", "uri": "../lciamethods/b2ad6110-c78d-11e6-9d9d-cec0c932ce01.xml"}, "other": {"anies": [{"name": "referenceToUnitGroupDataSet", "value": {"shortDescription": [{"value": "MJ", "lang": "en"}], "type": "unit group data set", "refObjectId": "93a60a57-a3c8-11da-a746-0800200c9a66", "uri": "../unitgroups/93a60a57-a3c8-11da-a746-0800200c9a66.xml"}}, {"value": "2805.36859018289", "module": "A1-A3"}, {"value": "40.199406572016", "module": "A4"}, {"value": "0.359554719506816", "module": "A5"}, {"value": "0", "module": "C1"}, {"value": "3.72970191692166", "module": "C2"}, {"value": "12.7676267311569", "module": "C3"}, {"value": "34.5672613973717", "module": "C4"}, {"value": "-683.404263667473", "module": "D", "scenario": "S1"}, {"value": "-28.99615012425", "module": "D", "scenario": "S2"}]}}, {"referenceToLCIAMethodDataSet": {"shortDescription": [{"value": "Water use (WDP)", "lang": "en"}, {"value": "Wassernutzung (WDP)", "lang": "de"}], "type": "LCIA method data set", "refObjectId": "b2ad66ce-c78d-11e6-9d9d-cec0c932ce01", "uri": "../lciamethods/b2ad66ce-c78d-11e6-9d9d-cec0c932ce01.xml"}, "other": {"anies": [{"name": "referenceToUnitGroupDataSet", "value": {"shortDescription": [{"value": "m^(3) world eq deprived", "lang": "en"}], "type": "unit group data set", "refObjectId": "6ae2df01-888e-46c8-b17d-49fa3869b476", "uri": "../unitgroups/6ae2df01-888e-46c8-b17d-49fa3869b476.xml"}}, {"value": "16.8765666958554", "module": "A1-A3"}, {"value": "0.0269825240415977", "module": "A4"}, {"value": "0.277639210446351", "module": "A5"}, {"value": "0", "module": "C1"}, {"value": "0.00250343923513019", "module": "C2"}, {"value": "0", "module": "C3"}, {"value": "-0.0240157391550966", "module": "C4"}, {"value": "-1.39874710389101", "module": "D", "scenario": "S1"}, {"value": "-0.0593834487103564", "module": "D", "scenario": "S2"}]}}, {"referenceToLCIAMethodDataSet": {"shortDescription": [{"value": "Incidence of disease due to PM emissions (PM)", "lang": "en"}, {"value": "Auftreten von Krankheiten aufgrund von Feinstaubemissionen (PM)", "lang": "de"}], "type": "LCIA method data set", "refObjectId": "b5c602c6-def3-11e6-bf01-fe55135034f3", "uri": "../lciamethods/b5c602c6-def3-11e6-bf01-fe55135034f3.xml"}, "other": {"anies": [{"name": "referenceToUnitGroupDataSet", "value": {"shortDescription": [{"value": "Disease incidence", "lang": "en"}], "type": "unit group data set", "refObjectId": "3883559b-648f-4afc-8ba2-0bd24f3affa3", "uri": "../unitgroups/3883559b-648f-4afc-8ba2-0bd24f3affa3.xml"}}, {"value": "1.13138948612618E-06", "module": "A1-A3"}, {"value": "1.74856244810853E-08", "module": "A4"}, {"value": "1.74532303575825E-09", "module": "A5"}, {"value": "0", "module": "C1"}, {"value": "1.62231666352695E-09", "module": "C2"}, {"value": "5.89561052901575E-08", "module": "C3"}, {"value": "6.93833590762066E-08", "module": "C4"}, {"value": "-3.24246571262392E-07", "module": "D", "scenario": "S1"}, {"value": "-1.37609795486667E-08", "module": "D", "scenario": "S2"}]}}, {"referenceToLCIAMethodDataSet": {"shortDescription": [{"value": "Human exposure efficiency relative to U235 (IR)", "lang": "en"}, {"value": "Wirkung durch Exposition des Menschen mit U235 (IR)", "lang": "de"}], "type": "LCIA method data set", "refObjectId": "b5c632be-def3-11e6-bf01-fe55135034f3", "uri": "../lciamethods/b5c632be-def3-11e6-bf01-fe55135034f3.xml"}, "other": {"anies": [{"name": "referenceToUnitGroupDataSet", "value": {"shortDescription": [{"value": "kBq U235 eq", "lang": "en"}], "type": "unit group data set", "refObjectId": "456b05bf-1415-44a9-9993-02452f554c09", "uri": "../unitgroups/456b05bf-1415-44a9-9993-02452f554c09.xml"}}, {"value": "8.33949437647806", "module": "A1-A3"}, {"value": "0.00727297661558876", "module": "A4"}, {"value": "0.00356249121633143", "module": "A5"}, {"value": "0", "module": "C1"}, {"value": "0.000674786946824509", "module": "C2"}, {"value": "0.125721960018526", "module": "C3"}, {"value": "0.0626928961000284", "module": "C4"}, {"value": "-9.33076933120484", "module": "D", "scenario": "S1"}, {"value": "-0.396155912493117", "module": "D", "scenario": "S2"}]}}, {"referenceToLCIAMethodDataSet": {"shortDescription": [{"value": "Comparative toxic unit for ecosystems (ETP-fw)", "lang": "en"}, {"value": "Toxizitätsvergleichseinheit für Ökosysteme (ETP-fw)", "lang": "de"}], "type": "LCIA method data set", "refObjectId": "ee1082d1-b0f7-43ca-a1f0-21e2a4a74511", "uri": "../lciamethods/ee1082d1-b0f7-43ca-a1f0-21e2a4a74511.xml"}, "other": {"anies": [{"name": "referenceToUnitGroupDataSet", "value": {"shortDescription": [{"value": "CTUe", "lang": "en"}], "type": "unit group data set", "refObjectId": "aa959ded-f1eb-4efb-9c5c-2d60be36b3e6", "uri": "../unitgroups/aa959ded-f1eb-4efb-9c5c-2d60be36b3e6.xml"}}, {"value": "1608.74439417145", "module": "A1-A3"}, {"value": "27.9091937193843", "module": "A4"}, {"value": "0.169346651088", "module": "A5"}, {"value": "0", "module": "C1"}, {"value": "2.58941567031458", "module": "C2"}, {"value": "6.26341767680077", "module": "C3"}, {"value": "33.8273013768935", "module": "C4"}, {"value": "-119.79195261532", "module": "D", "scenario": "S1"}, {"value": "-5.08585073550324", "module": "D", "scenario": "S2"}]}}, {"referenceToLCIAMethodDataSet": {"shortDescription": [{"value": "Comparative toxic unit for humans (carcinogenic) (HTP-c)", "lang": "en"}, {"value": "Toxizitätsvergleichseinheit für Menschen (krebserregend) (HTP-c)", "lang": "de"}], "type": "LCIA method data set", "refObjectId": "2299222a-bbd8-474f-9d4f-4dd1f18aea7c", "uri": "../lciamethods/2299222a-bbd8-474f-9d4f-4dd1f18aea7c.xml"}, "other": {"anies": [{"name": "referenceToUnitGroupDataSet", "value": {"shortDescription": [{"value": "CTUh", "lang": "en"}], "type": "unit group data set", "refObjectId": "d4c9523e-2d7e-49fd-8469-998f547d3a70", "uri": "../unitgroups/d4c9523e-2d7e-49fd-8469-998f547d3a70.xml"}}, {"value": "3.24350025273287E-08", "module": "A1-A3"}, {"value": "5.62472772966603E-10", "module": "A4"}, {"value": "1.89971260983824E-11", "module": "A5"}, {"value": "0", "module": "C1"}, {"value": "5.21862375204852E-11", "module": "C2"}, {"value": "6.31134213783169E-10", "module": "C3"}, {"value": "1.51891941087961E-09", "module": "C4"}, {"value": "-4.4650262410764E-09", "module": "D", "scenario": "S1"}, {"value": "-1.89424643105502E-10", "module": "D", "scenario": "S2"}]}}, {"referenceToLCIAMethodDataSet": {"shortDescription": [{"value": "Comparative toxic unit for humans (noncarcinogenic) (HTP-nc)", "lang": "en"}, {"value": "Toxizitätsvergleichseinheit für Menschen (nicht krebserregend) (HTP-nc)", "lang": "de"}], "type": "LCIA method data set", "refObjectId": "3af763a5-b7a1-48c9-9cee-1f223481fcef", "uri": "../lciamethods/3af763a5-b7a1-48c9-9cee-1f223481fcef.xml"}, "other": {"anies": [{"name": "referenceToUnitGroupDataSet", "value": {"shortDescription": [{"value": "CTUh", "lang": "en"}], "type": "unit group data set", "refObjectId": "d4c9523e-2d7e-49fd-8469-998f547d3a70", "uri": "../unitgroups/d4c9523e-2d7e-49fd-8469-998f547d3a70.xml"}}, {"value": "1.42188095056753E-06", "module": "A1-A3"}, {"value": "2.90732644755722E-08", "module": "A4"}, {"value": "5.99253374000661E-10", "module": "A5"}, {"value": "0", "module": "C1"}, {"value": "2.6974181833121E-09", "module": "C2"}, {"value": "2.05131871546431E-08", "module": "C3"}, {"value": "1.27303845579185E-07", "module": "C4"}, {"value": "-2.0508207833308E-07", "module": "D", "scenario": "S1"}, {"value": "-8.70109956165701E-09", "module": "D", "scenario": "S2"}]}}, {"referenceToLCIAMethodDataSet": {"shortDescription": [{"value": "Soil quality index (SQP)", "lang": "en"}, {"value": "Bodenqualitätsindex (SQP)", "lang": "de"}], "type": "LCIA method data set", "refObjectId": "b2ad6890-c78d-11e6-9d9d-cec0c932ce01", "uri": "../lciamethods/b2ad6890-c78d-11e6-9d9d-cec0c932ce01.xml"}, "other": {"anies": [{"name": "referenceToUnitGroupDataSet", "value": {"shortDescription": [{"value": "SQP", "lang": "en"}], "type": "unit group data set", "refObjectId": "f130951c-e67f-4f7f-8dd4-665de3974e18", "uri": "../unitgroups/f130951c-e67f-4f7f-8dd4-665de3974e18.xml"}}, {"value": "112.47049892904", "module": "A1-A3"}, {"value": "13.8325506745626", "module": "A4"}, {"value": "0.108915040820405", "module": "A5"}, {"value": "0", "module": "C1"}, {"value": "1.28338438714035", "module": "C2"}, {"value": "3.87936695552417", "module": "C3"}, {"value": "2.4871075085974", "module": "C4"}, {"value": "-35.8244744852197", "module": "D", "scenario": "S1"}, {"value": "-1.52095802967169", "module": "D", "scenario": "S2"}]}}]}, "otherAttributes": {"{http://www.indata.network/EPD/2019}epd-version": "1.2"}, "version": "1.1", "locations": "../ILCDLocations.xml"}