{"processInformation": {"dataSetInformation": {"UUID": "b5268215-2a5a-4516-a72f-3b53eda82ef1", "name": {"baseName": [{"value": "Sikaplan VGWT", "lang": "en"}, {"value": "Sikaplan VGWT", "lang": "de"}], "functionalUnitFlowProperties": [{"lang": "en"}]}, "classificationInformation": {"classification": [{"class": [{"value": "Kunststoffe", "level": 0, "classId": "6"}, {"value": "Dachbahnen", "level": 1, "classId": "6.3"}, {"value": "PVC-Dachbahnen", "level": 2, "classId": "6.3.02"}], "name": "OEKOBAU.DAT"}, {"class": [{"value": "02 Building products", "level": 0}, {"value": "Membranes, including Liquid applied and kits", "level": 1}, {"value": "Plastic and elastomer roofing and sealing sheet systems", "level": 2}], "name": "IBUCategories"}]}, "generalComment": [{"value": "Sikaplan VGWT is a multi-layer synthetic roof waterproofing sheet based on polyvinyl chloride (PVC) with embedded polyester scrim reinforcing (DE/E1 PVC-P-NB-V-PG).  \n\nSikaplan VGWT waterproofing sheets are available in these thicknesses: 1.2 mm, 1.5 mm and 1.8 mm.\n\nAll values given in the LCIA results section apply to Sikaplan VGWT-12; a formula for individually calculating values for other thicknesses is given in Chapter 5.\n\nPlacement of the product on the market in the European Union/European Free Trade Association (EU/EFTA) (except for Switzerland) is subject to Regulation (EU) No. 305/2011 (CPR). The product requires a Declaration of Performance in accordance with the harmonised standard EN 13956:2012 “Flexible sheets for waterproofing” and the CE marking. Application is subject to the regulations of each specific country; in Germany the application standard DIN SPEC 20000-201.", "lang": "en"}], "other": {"anies": [{"scenario": [{"description": [{"value": "Scenario 0", "lang": "en"}, {"value": "Szenario 0", "lang": "de"}], "name": "S0"}, {"description": [{"value": "100 % material recycling", "lang": "en"}, {"value": "100 % stoffliche Verwertung", "lang": "de"}], "name": "S1", "default": true}, {"description": [{"value": "100% thermal energy recovery", "lang": "en"}, {"value": "100 % thermische Energierückgewinnung", "lang": "de"}], "name": "S2"}]}]}}, "quantitativeReference": {"referenceToReferenceFlow": [0]}, "time": {"referenceYear": 2022, "dataSetValidUntil": 2027, "other": {"anies": [{"name": "publicationDateOfEPD", "value": 1669334400000}]}}, "geography": {"locationOfOperationSupplyOrProduction": {"location": "CH"}}, "technology": {"technologyDescriptionAndIncludedProcesses": [{"value": "Sikaplan VGWT polymeric waterproofing sheets are manufactured in the following steps: Dosing of the various raw materials and plastification of the mixture in an extruder Rolling the melt into sheets by calendar processing Cooling and reeling the sheets Heat fusing of two sheets (top and bottom layers), embedding a polyester mesh, on a lamination machine Trimming the sheets and winding them onto cardboard spools made of recycled paper Wrapping the rolls in PE stretch film, palletising Production waste such as scrap is recycled by feeding it directly back into the manufacturing process. Sika maintains a quality management system certified in accordance with ISO 9001. \nTechnical data: \nIn the following table, only technical data relevant to Sikaplan VGWT waterproofing sheets are given. \nDeclared unit: \nThis declaration applies to 1 m2 of Sikaplan VGWT polymeric waterproofing membrane, thickness 1.2 mm. A formula is given for an independent calculation of the values for other thicknesses.", "lang": "en"}, {"value": "Sikaplan VGWT Polymer-Abdichtungsbahnen werden in folgenden Schritten hergestellt:  \n\nDosierung der verschiedenen Rohstoffe und Plastifizierung der Mischung in einem Extruder\n\nWalzen der Schmelze zu Platten im Kalanderverfahren\n\nAbkühlen und Aufwickeln der Platten\n\nVerschmelzen von zwei Platten (Ober- und Unterschicht) unter Einbettung eines Polyestergewebes in einer Laminiermaschine\n\nSchneiden der Folien und Aufwickeln auf Kartonspulen aus Recyclingpapier\n\nEinwickeln der Rollen in PE-Stretchfolie, Palettierung \n\nProduktionsabfälle, wie z.B. Ausschuss, werden recycelt, indem sie direkt in den Herstellungsprozess zurückgeführt werden. \n\nSika unterhält ein nach ISO 9001 zertifiziertes Qualitätsmanagementsystem. \n", "lang": "de"}], "technologicalApplicability": [{"value": "Sikaplan VGWT waterproofing sheets are used mainly for waterproofing flat roofs. The sheets can be loosely laid and mechanically fastened to roofs with any slope.", "lang": "en"}, {"value": "Sikaplan VGWT Abdichtungsbahnen werden hauptsächlich für die Abdichtung von Flachdächern verwendet. Die Bahnen können auf Dächern mit beliebiger Neigung lose verlegt und mechanisch befestigt werden.", "lang": "de"}]}}, "modellingAndValidation": {"LCIMethodAndAllocation": {"typeOfDataSet": "EPD", "referenceToLCAMethodDetails": [{"shortDescription": [{"value": "Plastic and elastomer roofing and sealing sheet systems.pdf", "lang": "en"}], "type": "source data set", "refObjectId": "3cf9202c-ee26-4f5e-b281-7084dc4a041c"}], "other": {"anies": [{"name": "subType", "value": "specific dataset"}]}}, "dataSourcesTreatmentAndRepresentativeness": {"referenceToDataSource": [{"shortDescription": [{"value": "GaBi Database (all versions)", "lang": "en"}], "type": "source data set", "refObjectId": "28d74cc0-db8b-4d7e-bc44-5f6d56ce0c4a"}, {"shortDescription": [{"value": "GaBi Database Edition 2022, CUP 2022.01", "lang": "en"}], "type": "source data set", "refObjectId": "86f664e2-7dab-4722-aad7-4c5206a4123b"}], "useAdviceForDataSet": [{"value": "Scope: \nThis document applies to Sikaplan VGWT polymeric waterproofing membrane manufactured by Sika Manufacturing AG in Duedingen, Switzerland. The life cycle assessment data are based on production data from 2021 collected by Sika Services AG. \nSystem boundary: \nType of EPD: Cradle-to-gate with options\n\nThe system boundaries of the EPD follow the modular construction system described by EN 15804+A2. The LCA takes into account the following modules:\n\nA1-A3: Manufacturing of pre-products, packaging, ancillary materials, transport to the factory, production including energy supply and waste handling\nA4: Transport to the building site \nA5: Installation into the building (welding energy, disposal of packaging \nC1: Deconstruction and demolition\nC2/1: Transport to the recycling facility\nC2/2: Transport to the incineration facility\nC3/1: Waste processing for recycling\nC3/2: Waste incineration\nC4: Disposal \nD: Potential for reuse, recovery and/or recycling as net flows and benefits", "lang": "en"}], "other": {"anies": [{"name": "referenceToOriginalEPD", "value": {"shortDescription": {"value": "Sikaplan VGWT.pdf", "defaultValue": "Sikaplan VGWT.pdf", "lstrings": [{"lang": "en", "value": "Sikaplan VGWT.pdf"}]}, "type": "source data set", "uuid": {"uuid": "9248ad7d-554c-4c59-9ee0-0d64b01d40ef"}, "refObjectId": "9248ad7d-554c-4c59-9ee0-0d64b01d40ef", "resourceURLs": ["https://oekobaudat.de/OEKOBAU.DAT/resource/sources/9248ad7d-554c-4c59-9ee0-0d64b01d40ef/Sikaplan_VGWT_23268.pdf?version=00.03.000"]}}]}}, "validation": {"review": [{"referenceToNameOfReviewerAndInstitution": [{"shortDescription": [{"value": "Institut Bauen und Umwelt e. V.", "lang": "en"}], "type": "contact data set", "refObjectId": "d111dbec-b024-4be5-86c5-752d6eb2cf95", "uri": "../contacts/d111dbec-b024-4be5-86c5-752d6eb2cf95.xml"}], "type": "Accredited third party review"}]}, "complianceDeclarations": {"compliance": [{"referenceToComplianceSystem": {"shortDescription": [{"value": "DIN EN 15804+A2", "lang": "en"}], "type": "source data set", "refObjectId": "c0016b33-8cf7-415c-ac6e-deba0d21440d", "uri": "../sources/c0016b33-8cf7-415c-ac6e-deba0d21440d.xml"}}, {"referenceToComplianceSystem": {"shortDescription": [{"value": "ISO 14025", "lang": "en"}], "type": "source data set", "refObjectId": "4f2eb655-6e44-4874-a95a-e28f5442cd4d", "uri": "../sources/4f2eb655-6e44-4874-a95a-e28f5442cd4d.xml"}}]}}, "administrativeInformation": {"commissionerAndGoal": {"referenceToCommissioner": [{"shortDescription": [{"value": "Sika Deutschland GmbH", "lang": "en"}], "type": "contact data set", "refObjectId": "3d99c862-ca4d-4bff-9241-8a83668bd310", "uri": "../contacts/3d99c862-ca4d-4bff-9241-8a83668bd310.xml"}]}, "dataGenerator": {"referenceToPersonOrEntityGeneratingTheDataSet": [{"shortDescription": [{"value": "Sika Services AG", "lang": "en"}], "type": "contact data set", "refObjectId": "e6e310ee-d48d-41ec-b502-68ec650bae28", "uri": "../contacts/e6e310ee-d48d-41ec-b502-68ec650bae28.xml"}]}, "dataEntryBy": {"timeStamp": 1669365806736, "referenceToDataSetFormat": [{"shortDescription": [{"value": "ILCD Format", "lang": "en"}], "type": "source data set", "refObjectId": "a97a0155-0234-4b87-b4ce-a45da52f2a40", "uri": "../sources/a97a0155-0234-4b87-b4ce-a45da52f2a40.xml"}, {"shortDescription": [{"value": "EPD-Datenformaterweiterungen v1.2", "lang": "de"}, {"value": "EPD Data Format Extensions v1.2", "lang": "en"}], "type": "source data set", "refObjectId": "a29449fd-aa2f-4de8-b5d7-4b06b43c6fde", "uri": "../sources/a29449fd-aa2f-4de8-b5d7-4b06b43c6fde.xml"}]}, "publicationAndOwnership": {"dataSetVersion": "00.01.000", "referenceToPrecedingDataSetVersion": [{"shortDescription": [{"value": "Sikaplan VGWT", "lang": "en"}], "type": "process data set", "refObjectId": "aef41671-80ff-4ca6-9023-2bee20b33aed", "uri": "../processes/aef41671-80ff-4ca6-9023-2bee20b33aed.xml"}], "referenceToRegistrationAuthority": {"shortDescription": [{"value": "Institut Bauen und Umwelt e. V.", "lang": "en"}], "type": "contact data set", "refObjectId": "d111dbec-b024-4be5-86c5-752d6eb2cf95", "uri": "../contacts/d111dbec-b024-4be5-86c5-752d6eb2cf95.xml"}, "registrationNumber": "EPD-SIK-20220221-IBA1-EN", "referenceToOwnershipOfDataSet": {"shortDescription": [{"value": "Sika Deutschland GmbH", "lang": "en"}], "type": "contact data set", "refObjectId": "3d99c862-ca4d-4bff-9241-8a83668bd310", "uri": "../contacts/3d99c862-ca4d-4bff-9241-8a83668bd310.xml"}, "copyright": true, "licenseType": "Free of charge for all users and uses", "accessRestrictions": [{"value": "None", "lang": "en"}], "other": {"anies": [{"name": "referenceToPublisher", "value": {"shortDescription": [{"value": "Institut Bauen und Umwelt e. V.", "lang": "en"}], "type": "contact data set", "refObjectId": "d111dbec-b024-4be5-86c5-752d6eb2cf95", "uri": "../contacts/d111dbec-b024-4be5-86c5-752d6eb2cf95.xml"}}]}}}, "exchanges": {"exchange": [{"dataSetInternalID": 0, "referenceToFlowDataSet": {"shortDescription": [{"value": "Sikaplan VGWT-15 ()", "lang": "en"}], "type": "flow data set", "refObjectId": "5691a849-6304-a870-3d51-8304cbb71224", "uri": "../flows/5691a849-6304-a870-3d51-8304cbb71224.xml"}, "meanAmount": 1.0, "referencesToDataSource": {}, "referenceFlow": true, "resolvedFlowVersion": "00.01.000", "resultingflowAmount": 1.0, "flowProperties": [{"name": [{"lang": "en", "value": "Area"}, {"lang": "de", "value": "Fläche"}], "uuid": "93a60a56-a3c8-19da-a746-0800200c9a66", "referenceFlowProperty": true, "meanValue": 1.0, "referenceUnit": "qm", "unitGroupUUID": "c20a03d7-bd90-4569-bc94-66cfd364dfc8"}], "materialProperties": [{"name": "grammage", "value": "1.5", "unit": "kg/m^2", "unitDescription": "kilograms per square meter"}, {"name": "layer thickness", "value": "0.0015", "unit": "m", "unitDescription": "meters"}], "typeOfFlow": "Product flow", "classification": {"classHierarchy": "Kunststoffe / Dachbahnen / PVC-Dachbahnen", "name": "OEKOBAU.DAT"}}, {"dataSetInternalID": 1, "referenceToFlowDataSet": {"shortDescription": [{"value": "Renewable primary energy as energy carrier (PERE)", "lang": "en"}, {"value": "Erneuerbare Primärenergie als Energieträger (PERE)", "lang": "de"}], "type": "flow data set", "refObjectId": "20f32be5-0398-4288-9b6d-accddd195317", "uri": "../flows/20f32be5-0398-4288-9b6d-accddd195317.xml"}, "exchange direction": "INPUT", "other": {"anies": [{"name": "referenceToUnitGroupDataSet", "value": {"shortDescription": [{"value": "MJ", "lang": "en"}], "type": "unit group data set", "refObjectId": "93a60a57-a3c8-11da-a746-0800200c9a66", "uri": "../unitgroups/93a60a57-a3c8-11da-a746-0800200c9a66.xml"}}, {"value": "12.1597827490909", "module": "A1-A3"}, {"value": "0.0169090909090909", "module": "A4"}, {"value": "0.178266792145455", "module": "A5"}, {"value": "0", "module": "C1"}, {"value": "0.115", "module": "C2", "scenario": "S1"}, {"value": "0.0465", "module": "C2", "scenario": "S2"}, {"value": "0.768", "module": "C3", "scenario": "S1"}, {"value": "1.99", "module": "C3", "scenario": "S2"}, {"value": "0", "module": "C4"}, {"value": "-8.94", "module": "D", "scenario": "S1"}, {"value": "-6.53", "module": "D", "scenario": "S2"}]}, "resolvedFlowVersion": "38.00.000", "flowProperties": [], "typeOfFlow": "Other flow", "classification": {"classHierarchy": "Quantities", "name": "GaBiCategories"}}, {"dataSetInternalID": 2, "referenceToFlowDataSet": {"shortDescription": [{"value": "Renewable primary energy resources as material utilization (PERM)", "lang": "en"}, {"value": "Erneuerbare Primärenergie zur stofflichen Nutzung (PERM)", "lang": "de"}], "type": "flow data set", "refObjectId": "fb3ec0de-548d-4508-aea5-00b73bf6f702", "uri": "../flows/fb3ec0de-548d-4508-aea5-00b73bf6f702.xml"}, "exchange direction": "INPUT", "other": {"anies": [{"name": "referenceToUnitGroupDataSet", "value": {"shortDescription": [{"value": "MJ", "lang": "en"}], "type": "unit group data set", "refObjectId": "93a60a57-a3c8-11da-a746-0800200c9a66", "uri": "../unitgroups/93a60a57-a3c8-11da-a746-0800200c9a66.xml"}}, {"value": "1.74930816", "module": "A1-A3"}, {"value": "0", "module": "A4"}, {"value": "-0.0333958830545455", "module": "A5"}, {"value": "0", "module": "C1"}, {"value": "0", "module": "C2", "scenario": "S1"}, {"value": "0", "module": "C2", "scenario": "S2"}, {"value": "0", "module": "C3", "scenario": "S1"}, {"value": "0", "module": "C3", "scenario": "S2"}, {"value": "0", "module": "C4"}, {"value": "0", "module": "D", "scenario": "S1"}, {"value": "0", "module": "D", "scenario": "S2"}]}, "resolvedFlowVersion": "38.00.000", "flowProperties": [], "typeOfFlow": "Other flow", "classification": {"classHierarchy": "Quantities", "name": "GaBiCategories"}}, {"dataSetInternalID": 3, "referenceToFlowDataSet": {"shortDescription": [{"value": "Total use of renewable primary energy resources (PERT)", "lang": "en"}, {"value": "Total erneuerbare Primärenergie (PERT)", "lang": "de"}], "type": "flow data set", "refObjectId": "53f97275-fa8a-4cdd-9024-65936002acd0", "uri": "../flows/53f97275-fa8a-4cdd-9024-65936002acd0.xml"}, "exchange direction": "INPUT", "other": {"anies": [{"name": "referenceToUnitGroupDataSet", "value": {"shortDescription": [{"value": "MJ", "lang": "en"}], "type": "unit group data set", "refObjectId": "93a60a57-a3c8-11da-a746-0800200c9a66", "uri": "../unitgroups/93a60a57-a3c8-11da-a746-0800200c9a66.xml"}}, {"value": "13.9090909090909", "module": "A1-A3"}, {"value": "0.0169090909090909", "module": "A4"}, {"value": "0.144870909090909", "module": "A5"}, {"value": "0", "module": "C1"}, {"value": "0.115", "module": "C2", "scenario": "S1"}, {"value": "0.0465", "module": "C2", "scenario": "S2"}, {"value": "0.768", "module": "C3", "scenario": "S1"}, {"value": "1.99", "module": "C3", "scenario": "S2"}, {"value": "0", "module": "C4"}, {"value": "-8.94", "module": "D", "scenario": "S1"}, {"value": "-6.53", "module": "D", "scenario": "S2"}]}, "resolvedFlowVersion": "38.00.000", "flowProperties": [], "typeOfFlow": "Other flow", "classification": {"classHierarchy": "Quantities / Environmental quantities / EPD EN 15804 / LCI indicators", "name": "GaBiCategories"}}, {"dataSetInternalID": 4, "referenceToFlowDataSet": {"shortDescription": [{"value": "Non renewable primary energy as energy carrier (PENRE)", "lang": "en"}, {"value": "Nicht-erneuerbare Primärenergie als Energieträger (PENRE)", "lang": "de"}], "type": "flow data set", "refObjectId": "ac857178-2b45-46ec-892a-a9a4332f0372", "uri": "../flows/ac857178-2b45-46ec-892a-a9a4332f0372.xml"}, "exchange direction": "INPUT", "other": {"anies": [{"name": "referenceToUnitGroupDataSet", "value": {"shortDescription": [{"value": "MJ", "lang": "en"}], "type": "unit group data set", "refObjectId": "93a60a57-a3c8-11da-a746-0800200c9a66", "uri": "../unitgroups/93a60a57-a3c8-11da-a746-0800200c9a66.xml"}}, {"value": "58.6159452813853", "module": "A1-A3"}, {"value": "0.686363636363636", "module": "A4"}, {"value": "7.69115901952862", "module": "A5"}, {"value": "0", "module": "C1"}, {"value": "2.08", "module": "C2", "scenario": "S1"}, {"value": "0.82", "module": "C2", "scenario": "S2"}, {"value": "42.6138923636364", "module": "C3", "scenario": "S1"}, {"value": "49.1038923636364", "module": "C3", "scenario": "S2"}, {"value": "0", "module": "C4"}, {"value": "-68.6", "module": "D", "scenario": "S1"}, {"value": "-17", "module": "D", "scenario": "S2"}]}, "resolvedFlowVersion": "38.00.000", "flowProperties": [], "typeOfFlow": "Other flow", "classification": {"classHierarchy": "Quantities", "name": "GaBiCategories"}}, {"dataSetInternalID": 5, "referenceToFlowDataSet": {"shortDescription": [{"value": "Non renewable primary energy as material utilization (PENRM)", "lang": "en"}, {"value": "Nicht-erneuerbare Primärenergie zur stofflichen Nutzung (PENRM)", "lang": "de"}], "type": "flow data set", "refObjectId": "1421caa0-679d-4bf4-b282-0eb850ccae27", "uri": "../flows/1421caa0-679d-4bf4-b282-0eb850ccae27.xml"}, "exchange direction": "INPUT", "other": {"anies": [{"name": "referenceToUnitGroupDataSet", "value": {"shortDescription": [{"value": "MJ", "lang": "en"}], "type": "unit group data set", "refObjectId": "93a60a57-a3c8-11da-a746-0800200c9a66", "uri": "../unitgroups/93a60a57-a3c8-11da-a746-0800200c9a66.xml"}}, {"value": "40.4749638095238", "module": "A1-A3"}, {"value": "0", "module": "A4"}, {"value": "0.768551418181818", "module": "A5"}, {"value": "0", "module": "C1"}, {"value": "0", "module": "C2", "scenario": "S1"}, {"value": "0", "module": "C2", "scenario": "S2"}, {"value": "-41.6138923636364", "module": "C3", "scenario": "S1"}, {"value": "-41.6138923636364", "module": "C3", "scenario": "S2"}, {"value": "0", "module": "C4"}, {"value": "0", "module": "D", "scenario": "S1"}, {"value": "0", "module": "D", "scenario": "S2"}]}, "resolvedFlowVersion": "38.00.000", "flowProperties": [], "typeOfFlow": "Other flow", "classification": {"classHierarchy": "Quantities", "name": "GaBiCategories"}}, {"dataSetInternalID": 6, "referenceToFlowDataSet": {"shortDescription": [{"value": "Total use of non renewable primary energy resources (PENRT)", "lang": "en"}, {"value": "Total nicht erneuerbare Primärenergie (PENRT)", "lang": "de"}], "type": "flow data set", "refObjectId": "06159210-646b-4c8d-8583-da9b3b95a6c1", "uri": "../flows/06159210-646b-4c8d-8583-da9b3b95a6c1.xml"}, "exchange direction": "INPUT", "other": {"anies": [{"name": "referenceToUnitGroupDataSet", "value": {"shortDescription": [{"value": "MJ", "lang": "en"}], "type": "unit group data set", "refObjectId": "93a60a57-a3c8-11da-a746-0800200c9a66", "uri": "../unitgroups/93a60a57-a3c8-11da-a746-0800200c9a66.xml"}}, {"value": "99.0909090909091", "module": "A1-A3"}, {"value": "0.686363636363636", "module": "A4"}, {"value": "8.45971043771044", "module": "A5"}, {"value": "0", "module": "C1"}, {"value": "2.08", "module": "C2", "scenario": "S1"}, {"value": "0.82", "module": "C2", "scenario": "S2"}, {"value": "1", "module": "C3", "scenario": "S1"}, {"value": "7.49", "module": "C3", "scenario": "S2"}, {"value": "0", "module": "C4"}, {"value": "-68.6", "module": "D", "scenario": "S1"}, {"value": "-17", "module": "D", "scenario": "S2"}]}, "resolvedFlowVersion": "38.00.000", "flowProperties": [], "typeOfFlow": "Other flow", "classification": {"classHierarchy": "Quantities / Environmental quantities / EPD EN 15804 / LCI indicators", "name": "GaBiCategories"}}, {"dataSetInternalID": 7, "referenceToFlowDataSet": {"shortDescription": [{"value": "Use of secondary material (SM)", "lang": "en"}, {"value": "Einsatz von Sekundärstoffen (SM)", "lang": "de"}], "type": "flow data set", "refObjectId": "c6a1f35f-2d09-4f54-8dfb-97e502e1ce92", "uri": "../flows/c6a1f35f-2d09-4f54-8dfb-97e502e1ce92.xml"}, "exchange direction": "INPUT", "other": {"anies": [{"name": "referenceToUnitGroupDataSet", "value": {"shortDescription": [{"value": "kg", "lang": "en"}], "type": "unit group data set", "refObjectId": "ad38d542-3fe9-439d-9b95-2f5f7752acaf", "uri": "../unitgroups/ad38d542-3fe9-439d-9b95-2f5f7752acaf.xml"}}, {"value": "0.0545454545454545", "module": "A1-A3"}, {"value": "0", "module": "A4"}, {"value": "0.00545454545454545", "module": "A5"}, {"value": "0", "module": "C1"}, {"value": "0", "module": "C2", "scenario": "S1"}, {"value": "0", "module": "C2", "scenario": "S2"}, {"value": "0", "module": "C3", "scenario": "S1"}, {"value": "0", "module": "C3", "scenario": "S2"}, {"value": "0", "module": "C4"}, {"value": "-1.54", "module": "D", "scenario": "S1"}, {"value": "0", "module": "D", "scenario": "S2"}]}, "resolvedFlowVersion": "38.00.000", "flowProperties": [], "typeOfFlow": "Other flow", "classification": {"classHierarchy": "Quantities / Environmental quantities / EPD EN 15804 / LCI indicators", "name": "GaBiCategories"}}, {"dataSetInternalID": 8, "referenceToFlowDataSet": {"shortDescription": [{"value": "Use of renewable secondary fuels (RSF)", "lang": "en"}, {"value": "Erneuerbare Sekundärbrennstoffe (RSF)", "lang": "de"}], "type": "flow data set", "refObjectId": "64333088-a55f-4aa2-9a31-c10b07816787", "uri": "../flows/64333088-a55f-4aa2-9a31-c10b07816787.xml"}, "exchange direction": "INPUT", "other": {"anies": [{"name": "referenceToUnitGroupDataSet", "value": {"shortDescription": [{"value": "MJ", "lang": "en"}], "type": "unit group data set", "refObjectId": "93a60a57-a3c8-11da-a746-0800200c9a66", "uri": "../unitgroups/93a60a57-a3c8-11da-a746-0800200c9a66.xml"}}, {"value": "0", "module": "A1-A3"}, {"value": "0", "module": "A4"}, {"value": "0", "module": "A5"}, {"value": "0", "module": "C1"}, {"value": "0", "module": "C2", "scenario": "S1"}, {"value": "0", "module": "C2", "scenario": "S2"}, {"value": "0", "module": "C3", "scenario": "S1"}, {"value": "0", "module": "C3", "scenario": "S2"}, {"value": "0", "module": "C4"}, {"value": "0", "module": "D", "scenario": "S1"}, {"value": "0", "module": "D", "scenario": "S2"}]}, "resolvedFlowVersion": "38.00.000", "flowProperties": [], "typeOfFlow": "Other flow", "classification": {"classHierarchy": "Quantities / Environmental quantities / EPD EN 15804 / LCI indicators", "name": "GaBiCategories"}}, {"dataSetInternalID": 9, "referenceToFlowDataSet": {"shortDescription": [{"value": "Use of non renewable secondary fuels (NRSF)", "lang": "en"}, {"value": "Nicht erneuerbare Sekundärbrennstoffe (NRSF)", "lang": "de"}], "type": "flow data set", "refObjectId": "89def144-d39a-4287-b86f-efde453ddcb2", "uri": "../flows/89def144-d39a-4287-b86f-efde453ddcb2.xml"}, "exchange direction": "INPUT", "other": {"anies": [{"name": "referenceToUnitGroupDataSet", "value": {"shortDescription": [{"value": "MJ", "lang": "en"}], "type": "unit group data set", "refObjectId": "93a60a57-a3c8-11da-a746-0800200c9a66", "uri": "../unitgroups/93a60a57-a3c8-11da-a746-0800200c9a66.xml"}}, {"value": "0", "module": "A1-A3"}, {"value": "0", "module": "A4"}, {"value": "0", "module": "A5"}, {"value": "0", "module": "C1"}, {"value": "0", "module": "C2", "scenario": "S1"}, {"value": "0", "module": "C2", "scenario": "S2"}, {"value": "0", "module": "C3", "scenario": "S1"}, {"value": "0", "module": "C3", "scenario": "S2"}, {"value": "0", "module": "C4"}, {"value": "0", "module": "D", "scenario": "S1"}, {"value": "0", "module": "D", "scenario": "S2"}]}, "resolvedFlowVersion": "38.00.000", "flowProperties": [], "typeOfFlow": "Other flow", "classification": {"classHierarchy": "Quantities / Environmental quantities / EPD EN 15804 / LCI indicators", "name": "GaBiCategories"}}, {"dataSetInternalID": 10, "referenceToFlowDataSet": {"shortDescription": [{"value": "Use of net fresh water (FW)", "lang": "en"}, {"value": "Einsatz von Süßwasserressourcen (FW)", "lang": "de"}], "type": "flow data set", "refObjectId": "3cf952c8-f3a4-461d-8c96-96456ca62246", "uri": "../flows/3cf952c8-f3a4-461d-8c96-96456ca62246.xml"}, "exchange direction": "INPUT", "other": {"anies": [{"name": "referenceToUnitGroupDataSet", "value": {"shortDescription": [{"value": "m^3", "lang": "en"}], "type": "unit group data set", "refObjectId": "cd950537-0a98-4044-9ba7-9f9a68d0a504", "uri": "../unitgroups/cd950537-0a98-4044-9ba7-9f9a68d0a504.xml"}}, {"value": "0.0254545454545455", "module": "A1-A3"}, {"value": "1.59090909090909E-05", "module": "A4"}, {"value": "0.00323504545454545", "module": "A5"}, {"value": "0", "module": "C1"}, {"value": "0.000131", "module": "C2", "scenario": "S1"}, {"value": "5.26E-05", "module": "C2", "scenario": "S2"}, {"value": "0.000607", "module": "C3", "scenario": "S1"}, {"value": "0.00847", "module": "C3", "scenario": "S2"}, {"value": "0", "module": "C4"}, {"value": "-0.0118", "module": "D", "scenario": "S1"}, {"value": "-0.00267", "module": "D", "scenario": "S2"}]}, "resolvedFlowVersion": "38.00.000", "flowProperties": [], "typeOfFlow": "Other flow", "classification": {"classHierarchy": "Quantities / Environmental quantities / EPD EN 15804 / LCI indicators", "name": "GaBiCategories"}}, {"dataSetInternalID": 11, "referenceToFlowDataSet": {"shortDescription": [{"value": "Hazardous waste disposed (HWD)", "lang": "en"}, {"value": "Gefährlicher Abfall zur Deponie (HWD)", "lang": "de"}], "type": "flow data set", "refObjectId": "430f9e0f-59b2-46a0-8e0d-55e0e84948fc", "uri": "../flows/430f9e0f-59b2-46a0-8e0d-55e0e84948fc.xml"}, "exchange direction": "OUTPUT", "other": {"anies": [{"name": "referenceToUnitGroupDataSet", "value": {"shortDescription": [{"value": "kg", "lang": "en"}], "type": "unit group data set", "refObjectId": "ad38d542-3fe9-439d-9b95-2f5f7752acaf", "uri": "../unitgroups/ad38d542-3fe9-439d-9b95-2f5f7752acaf.xml"}}, {"value": "7.75454545454545E-07", "module": "A1-A3"}, {"value": "2.93636363636364E-12", "module": "A4"}, {"value": "7.75718481818182E-08", "module": "A5"}, {"value": "0", "module": "C1"}, {"value": "9.91E-12", "module": "C2", "scenario": "S1"}, {"value": "3.93E-12", "module": "C2", "scenario": "S2"}, {"value": "1.04E-10", "module": "C3", "scenario": "S1"}, {"value": "5.81E-10", "module": "C3", "scenario": "S2"}, {"value": "0", "module": "C4"}, {"value": "-1.43E-06", "module": "D", "scenario": "S1"}, {"value": "-2.83E-09", "module": "D", "scenario": "S2"}]}, "resolvedFlowVersion": "38.00.000", "flowProperties": [], "typeOfFlow": "Other flow", "classification": {"classHierarchy": "Quantities / Environmental quantities / EPD EN 15804 / LCI indicators", "name": "GaBiCategories"}}, {"dataSetInternalID": 12, "referenceToFlowDataSet": {"shortDescription": [{"value": "Non hazardous waste disposed (NHWD)", "lang": "en"}, {"value": "Entsorgter nicht gefährlicher Abfall (NHWD)", "lang": "de"}], "type": "flow data set", "refObjectId": "b29ef66b-e286-4afa-949f-62f1a7b4d7fa", "uri": "../flows/b29ef66b-e286-4afa-949f-62f1a7b4d7fa.xml"}, "exchange direction": "OUTPUT", "other": {"anies": [{"name": "referenceToUnitGroupDataSet", "value": {"shortDescription": [{"value": "kg", "lang": "en"}], "type": "unit group data set", "refObjectId": "ad38d542-3fe9-439d-9b95-2f5f7752acaf", "uri": "../unitgroups/ad38d542-3fe9-439d-9b95-2f5f7752acaf.xml"}}, {"value": "0.215454545454545", "module": "A1-A3"}, {"value": "8.10909090909091E-05", "module": "A4"}, {"value": "0.0718535636363636", "module": "A5"}, {"value": "0", "module": "C1"}, {"value": "0.000295", "module": "C2", "scenario": "S1"}, {"value": "0.000117", "module": "C2", "scenario": "S2"}, {"value": "0.0149", "module": "C3", "scenario": "S1"}, {"value": "2.58", "module": "C3", "scenario": "S2"}, {"value": "0", "module": "C4"}, {"value": "-0.033", "module": "D", "scenario": "S1"}, {"value": "-0.0106", "module": "D", "scenario": "S2"}]}, "resolvedFlowVersion": "38.00.000", "flowProperties": [], "typeOfFlow": "Other flow", "classification": {"classHierarchy": "Quantities / Environmental quantities / EPD EN 15804 / LCI indicators", "name": "GaBiCategories"}}, {"dataSetInternalID": 13, "referenceToFlowDataSet": {"shortDescription": [{"value": "Radioactive waste disposed (RWD)", "lang": "en"}, {"value": "Entsorgter radioaktiver Abfall (RWD)", "lang": "de"}], "type": "flow data set", "refObjectId": "3449546e-52ad-4b39-b809-9fb77cea8ff6", "uri": "../flows/3449546e-52ad-4b39-b809-9fb77cea8ff6.xml"}, "exchange direction": "OUTPUT", "other": {"anies": [{"name": "referenceToUnitGroupDataSet", "value": {"shortDescription": [{"value": "kg", "lang": "en"}], "type": "unit group data set", "refObjectId": "ad38d542-3fe9-439d-9b95-2f5f7752acaf", "uri": "../unitgroups/ad38d542-3fe9-439d-9b95-2f5f7752acaf.xml"}}, {"value": "0.00213636363636364", "module": "A1-A3"}, {"value": "7.47272727272727E-07", "module": "A4"}, {"value": "0.000241211090909091", "module": "A5"}, {"value": "0", "module": "C1"}, {"value": "2.55E-06", "module": "C2", "scenario": "S1"}, {"value": "1.01E-06", "module": "C2", "scenario": "S2"}, {"value": "8.6E-05", "module": "C3", "scenario": "S1"}, {"value": "0.000236", "module": "C3", "scenario": "S2"}, {"value": "0", "module": "C4"}, {"value": "-0.00132", "module": "D", "scenario": "S1"}, {"value": "-0.000721", "module": "D", "scenario": "S2"}]}, "resolvedFlowVersion": "38.00.000", "flowProperties": [], "typeOfFlow": "Other flow", "classification": {"classHierarchy": "Quantities / Environmental quantities / EPD EN 15804 / LCI indicators", "name": "GaBiCategories"}}, {"dataSetInternalID": 14, "referenceToFlowDataSet": {"shortDescription": [{"value": "Components for re-use (CRU)", "lang": "en"}, {"value": "Komponenten für die Wiederverwendung (CRU)", "lang": "de"}], "type": "flow data set", "refObjectId": "a2b32f97-3fc7-4af2-b209-525bc6426f33", "uri": "../flows/a2b32f97-3fc7-4af2-b209-525bc6426f33.xml"}, "exchange direction": "OUTPUT", "other": {"anies": [{"name": "referenceToUnitGroupDataSet", "value": {"shortDescription": [{"value": "kg", "lang": "en"}], "type": "unit group data set", "refObjectId": "ad38d542-3fe9-439d-9b95-2f5f7752acaf", "uri": "../unitgroups/ad38d542-3fe9-439d-9b95-2f5f7752acaf.xml"}}, {"value": "0", "module": "A1-A3"}, {"value": "0", "module": "A4"}, {"value": "0", "module": "A5"}, {"value": "0", "module": "C1"}, {"value": "0", "module": "C2", "scenario": "S1"}, {"value": "0", "module": "C2", "scenario": "S2"}, {"value": "0", "module": "C3", "scenario": "S1"}, {"value": "0", "module": "C3", "scenario": "S2"}, {"value": "0", "module": "C4"}, {"value": "0", "module": "D", "scenario": "S1"}, {"value": "0", "module": "D", "scenario": "S2"}]}, "resolvedFlowVersion": "38.00.000", "flowProperties": [], "typeOfFlow": "Other flow", "classification": {"classHierarchy": "Quantities / Environmental quantities / EPD EN 15804 / LCI indicators", "name": "GaBiCategories"}}, {"dataSetInternalID": 15, "referenceToFlowDataSet": {"shortDescription": [{"value": "Materials for recycling (MFR)", "lang": "en"}, {"value": "Stoffe zum Recycling (MFR)", "lang": "de"}], "type": "flow data set", "refObjectId": "d7fe48a5-4103-49c8-9aae-b0b5dfdbd6ae", "uri": "../flows/d7fe48a5-4103-49c8-9aae-b0b5dfdbd6ae.xml"}, "exchange direction": "OUTPUT", "other": {"anies": [{"name": "referenceToUnitGroupDataSet", "value": {"shortDescription": [{"value": "kg", "lang": "en"}], "type": "unit group data set", "refObjectId": "ad38d542-3fe9-439d-9b95-2f5f7752acaf", "uri": "../unitgroups/ad38d542-3fe9-439d-9b95-2f5f7752acaf.xml"}}, {"value": "0", "module": "A1-A3"}, {"value": "0", "module": "A4"}, {"value": "0", "module": "A5"}, {"value": "0", "module": "C1"}, {"value": "0", "module": "C2", "scenario": "S1"}, {"value": "0", "module": "C2", "scenario": "S2"}, {"value": "1.54", "module": "C3", "scenario": "S1"}, {"value": "0", "module": "C3", "scenario": "S2"}, {"value": "0", "module": "C4"}, {"value": "0", "module": "D", "scenario": "S1"}, {"value": "0", "module": "D", "scenario": "S2"}]}, "resolvedFlowVersion": "38.00.000", "flowProperties": [], "typeOfFlow": "Other flow", "classification": {"classHierarchy": "Quantities / Environmental quantities / EPD EN 15804 / LCI indicators", "name": "GaBiCategories"}}, {"dataSetInternalID": 16, "referenceToFlowDataSet": {"shortDescription": [{"value": "Materials for energy recovery (MER)", "lang": "en"}, {"value": "Stoffe für die Energierückgewinnung (MER)", "lang": "de"}], "type": "flow data set", "refObjectId": "59a9181c-3aaf-46ee-8b13-2b3723b6e447", "uri": "../flows/59a9181c-3aaf-46ee-8b13-2b3723b6e447.xml"}, "exchange direction": "OUTPUT", "other": {"anies": [{"name": "referenceToUnitGroupDataSet", "value": {"shortDescription": [{"value": "kg", "lang": "en"}], "type": "unit group data set", "refObjectId": "ad38d542-3fe9-439d-9b95-2f5f7752acaf", "uri": "../unitgroups/ad38d542-3fe9-439d-9b95-2f5f7752acaf.xml"}}, {"value": "0", "module": "A1-A3"}, {"value": "0", "module": "A4"}, {"value": "0", "module": "A5"}, {"value": "0", "module": "C1"}, {"value": "0", "module": "C2", "scenario": "S1"}, {"value": "0", "module": "C2", "scenario": "S2"}, {"value": "0", "module": "C3", "scenario": "S1"}, {"value": "0", "module": "C3", "scenario": "S2"}, {"value": "0", "module": "C4"}, {"value": "0", "module": "D", "scenario": "S1"}, {"value": "0", "module": "D", "scenario": "S2"}]}, "resolvedFlowVersion": "38.00.000", "flowProperties": [], "typeOfFlow": "Other flow", "classification": {"classHierarchy": "Quantities / Environmental quantities / EPD EN 15804 / LCI indicators", "name": "GaBiCategories"}}, {"dataSetInternalID": 17, "referenceToFlowDataSet": {"shortDescription": [{"value": "Exported electrical energy (EEE)", "lang": "en"}, {"value": "Exportierte elektrische Energie (EEE)", "lang": "de"}], "type": "flow data set", "refObjectId": "4da0c987-2b76-40d6-9e9e-82a017aaaf29", "uri": "../flows/4da0c987-2b76-40d6-9e9e-82a017aaaf29.xml"}, "exchange direction": "OUTPUT", "other": {"anies": [{"name": "referenceToUnitGroupDataSet", "value": {"shortDescription": [{"value": "MJ", "lang": "en"}], "type": "unit group data set", "refObjectId": "93a60a57-a3c8-11da-a746-0800200c9a66", "uri": "../unitgroups/93a60a57-a3c8-11da-a746-0800200c9a66.xml"}}, {"value": "0", "module": "A1-A3"}, {"value": "0", "module": "A4"}, {"value": "0.349", "module": "A5"}, {"value": "0", "module": "C1"}, {"value": "0", "module": "C2", "scenario": "S1"}, {"value": "0", "module": "C2", "scenario": "S2"}, {"value": "0.114", "module": "C3", "scenario": "S1"}, {"value": "4.23", "module": "C3", "scenario": "S2"}, {"value": "0", "module": "C4"}, {"value": "0", "module": "D", "scenario": "S1"}, {"value": "0", "module": "D", "scenario": "S2"}]}, "resolvedFlowVersion": "38.00.000", "flowProperties": [], "typeOfFlow": "Other flow", "classification": {"classHierarchy": "Quantities / Environmental quantities / EPD EN 15804 / LCI indicators", "name": "GaBiCategories"}}, {"dataSetInternalID": 18, "referenceToFlowDataSet": {"shortDescription": [{"value": "Exported thermal energy (EET)", "lang": "en"}, {"value": "Exportierte thermische Energie (EET)", "lang": "de"}], "type": "flow data set", "refObjectId": "98daf38a-7a79-46d3-9a37-2b7bd0955810", "uri": "../flows/98daf38a-7a79-46d3-9a37-2b7bd0955810.xml"}, "exchange direction": "OUTPUT", "other": {"anies": [{"name": "referenceToUnitGroupDataSet", "value": {"shortDescription": [{"value": "MJ", "lang": "en"}], "type": "unit group data set", "refObjectId": "93a60a57-a3c8-11da-a746-0800200c9a66", "uri": "../unitgroups/93a60a57-a3c8-11da-a746-0800200c9a66.xml"}}, {"value": "0", "module": "A1-A3"}, {"value": "0", "module": "A4"}, {"value": "0.629", "module": "A5"}, {"value": "0", "module": "C1"}, {"value": "0", "module": "C2", "scenario": "S1"}, {"value": "0", "module": "C2", "scenario": "S2"}, {"value": "0.213", "module": "C3", "scenario": "S1"}, {"value": "7.72", "module": "C3", "scenario": "S2"}, {"value": "0", "module": "C4"}, {"value": "0", "module": "D", "scenario": "S1"}, {"value": "0", "module": "D", "scenario": "S2"}]}, "resolvedFlowVersion": "38.00.000", "flowProperties": [], "typeOfFlow": "Other flow", "classification": {"classHierarchy": "Quantities / Environmental quantities / EPD EN 15804 / LCI indicators", "name": "GaBiCategories"}}]}, "LCIAResults": {"LCIAResult": [{"referenceToLCIAMethodDataSet": {"shortDescription": [{"value": "Global Warming Potential total (GWP-total)", "lang": "en"}, {"value": "Globales Erwärmungspotenzial total (GWP-total)", "lang": "de"}], "type": "LCIA method data set", "refObjectId": "6a37f984-a4b3-458a-a20a-64418c145fa2", "uri": "../lciamethods/6a37f984-a4b3-458a-a20a-64418c145fa2.xml"}, "other": {"anies": [{"name": "referenceToUnitGroupDataSet", "value": {"shortDescription": [{"value": "kg CO_(2)-Äq.", "lang": "en"}], "type": "unit group data set", "refObjectId": "1ebf3012-d0db-4de2-aefd-ef30cedb0be1", "uri": "../unitgroups/1ebf3012-d0db-4de2-aefd-ef30cedb0be1.xml"}}, {"value": "4.17272727272727", "module": "A1-A3"}, {"value": "0.0549090909090909", "module": "A4"}, {"value": "0.689763636363636", "module": "A5"}, {"value": "0", "module": "C1"}, {"value": "0.0195", "module": "C2", "scenario": "S1"}, {"value": "0.0064", "module": "C2", "scenario": "S2"}, {"value": "0.234", "module": "C3", "scenario": "S1"}, {"value": "4.23", "module": "C3", "scenario": "S2"}, {"value": "0", "module": "C4"}, {"value": "-2.85", "module": "D", "scenario": "S1"}, {"value": "-1.2", "module": "D", "scenario": "S2"}]}}, {"referenceToLCIAMethodDataSet": {"shortDescription": [{"value": "Global Warming Potential fossil fuels (GWP-fossil)", "lang": "en"}, {"value": "Globales Erwärmungspotenzial fossil (GWP-fossil)", "lang": "de"}], "type": "LCIA method data set", "refObjectId": "5f635281-343e-44fb-83df-1971b155e6b6", "uri": "../lciamethods/5f635281-343e-44fb-83df-1971b155e6b6.xml"}, "other": {"anies": [{"name": "referenceToUnitGroupDataSet", "value": {"shortDescription": [{"value": "kg CO_(2)-Äq.", "lang": "en"}], "type": "unit group data set", "refObjectId": "1ebf3012-d0db-4de2-aefd-ef30cedb0be1", "uri": "../unitgroups/1ebf3012-d0db-4de2-aefd-ef30cedb0be1.xml"}}, {"value": "4.35454545454545", "module": "A1-A3"}, {"value": "0.0548181818181818", "module": "A4"}, {"value": "0.537536363636364", "module": "A5"}, {"value": "0", "module": "C1"}, {"value": "0.0256", "module": "C2", "scenario": "S1"}, {"value": "0.00886", "module": "C2", "scenario": "S2"}, {"value": "0.23", "module": "C3", "scenario": "S1"}, {"value": "4.23", "module": "C3", "scenario": "S2"}, {"value": "0", "module": "C4"}, {"value": "-2.82", "module": "D", "scenario": "S1"}, {"value": "-1.19", "module": "D", "scenario": "S2"}]}}, {"referenceToLCIAMethodDataSet": {"shortDescription": [{"value": "Global Warming Potential biogenic (GWP-biogenic)", "lang": "en"}, {"value": "Globales Erwärmungspotenzial biogen (GWP-biogenic)", "lang": "de"}], "type": "LCIA method data set", "refObjectId": "2356e1ab-0185-4db5-86e5-16de51c7485c", "uri": "../lciamethods/2356e1ab-0185-4db5-86e5-16de51c7485c.xml"}, "other": {"anies": [{"name": "referenceToUnitGroupDataSet", "value": {"shortDescription": [{"value": "kg CO_(2)-Äq.", "lang": "en"}], "type": "unit group data set", "refObjectId": "1ebf3012-d0db-4de2-aefd-ef30cedb0be1", "uri": "../unitgroups/1ebf3012-d0db-4de2-aefd-ef30cedb0be1.xml"}}, {"value": "-0.250909090909091", "module": "A1-A3"}, {"value": "5.03636363636364E-05", "module": "A4"}, {"value": "0.144914127272727", "module": "A5"}, {"value": "0", "module": "C1"}, {"value": "-0.00695", "module": "C2", "scenario": "S1"}, {"value": "-0.0028", "module": "C2", "scenario": "S2"}, {"value": "0.00369", "module": "C3", "scenario": "S1"}, {"value": "0.00333", "module": "C3", "scenario": "S2"}, {"value": "0", "module": "C4"}, {"value": "-0.0229", "module": "D", "scenario": "S1"}, {"value": "-0.00952", "module": "D", "scenario": "S2"}]}}, {"referenceToLCIAMethodDataSet": {"shortDescription": [{"value": "Global Warming Potential luluc (GWP-luluc)", "lang": "en"}, {"value": "Globales Erwärmungspotenzial luluc (GWP-luluc)", "lang": "de"}], "type": "LCIA method data set", "refObjectId": "4331bbdb-978a-490d-8707-eeb047f01a55", "uri": "../lciamethods/4331bbdb-978a-490d-8707-eeb047f01a55.xml"}, "other": {"anies": [{"name": "referenceToUnitGroupDataSet", "value": {"shortDescription": [{"value": "kg CO_(2)-Äq.", "lang": "en"}], "type": "unit group data set", "refObjectId": "1ebf3012-d0db-4de2-aefd-ef30cedb0be1", "uri": "../unitgroups/1ebf3012-d0db-4de2-aefd-ef30cedb0be1.xml"}}, {"value": "0.0632727272727273", "module": "A1-A3"}, {"value": "7.23636363636364E-05", "module": "A4"}, {"value": "0.00634540909090909", "module": "A5"}, {"value": "0", "module": "C1"}, {"value": "0.000846", "module": "C2", "scenario": "S1"}, {"value": "0.000341", "module": "C2", "scenario": "S2"}, {"value": "2.65E-05", "module": "C3", "scenario": "S1"}, {"value": "0.000326", "module": "C3", "scenario": "S2"}, {"value": "0", "module": "C4"}, {"value": "-0.00171", "module": "D", "scenario": "S1"}, {"value": "-0.00023", "module": "D", "scenario": "S2"}]}}, {"referenceToLCIAMethodDataSet": {"shortDescription": [{"value": "Depletion potential of the stratospheric ozone layer (ODP)", "lang": "en"}, {"value": "Abbau Potential der stratosphärischen Ozonschicht (ODP)", "lang": "de"}], "type": "LCIA method data set", "refObjectId": "b5c629d6-def3-11e6-bf01-fe55135034f3", "uri": "../lciamethods/b5c629d6-def3-11e6-bf01-fe55135034f3.xml"}, "other": {"anies": [{"name": "referenceToUnitGroupDataSet", "value": {"shortDescription": [{"value": "kg CFC11-Äq.", "lang": "en"}], "type": "unit group data set", "refObjectId": "d9e957c9-7309-4474-bf3a-7777df6c4e5b", "uri": "../unitgroups/d9e957c9-7309-4474-bf3a-7777df6c4e5b.xml"}}, {"value": "4.56363636363636E-09", "module": "A1-A3"}, {"value": "4.79090909090909E-15", "module": "A4"}, {"value": "4.56559115454545E-10", "module": "A5"}, {"value": "0", "module": "C1"}, {"value": "9.3E-15", "module": "C2", "scenario": "S1"}, {"value": "3.67E-15", "module": "C2", "scenario": "S2"}, {"value": "1.65E-12", "module": "C3", "scenario": "S1"}, {"value": "4.04E-12", "module": "C3", "scenario": "S2"}, {"value": "0", "module": "C4"}, {"value": "-2E-10", "module": "D", "scenario": "S1"}, {"value": "-1.4E-11", "module": "D", "scenario": "S2"}]}}, {"referenceToLCIAMethodDataSet": {"shortDescription": [{"value": "Acidification potential of land and water (AP)", "lang": "en"}, {"value": "Versauerungspotenzial von Boden und Wasser (AP)", "lang": "de"}], "type": "LCIA method data set", "refObjectId": "b5c611c6-def3-11e6-bf01-fe55135034f3", "uri": "../lciamethods/b5c611c6-def3-11e6-bf01-fe55135034f3.xml"}, "other": {"anies": [{"name": "referenceToUnitGroupDataSet", "value": {"shortDescription": [{"value": "mol H^(+)-Äq.", "lang": "en"}], "type": "unit group data set", "refObjectId": "42e089ac-92bf-4bf2-8ca1-5fc40d18f2ed", "uri": "../unitgroups/42e089ac-92bf-4bf2-8ca1-5fc40d18f2ed.xml"}}, {"value": "0.0459090909090909", "module": "A1-A3"}, {"value": "0.00137272727272727", "module": "A4"}, {"value": "0.00479648181818182", "module": "A5"}, {"value": "0", "module": "C1"}, {"value": "0.000227", "module": "C2", "scenario": "S1"}, {"value": "3.62E-05", "module": "C2", "scenario": "S2"}, {"value": "0.000183", "module": "C3", "scenario": "S1"}, {"value": "0.00109", "module": "C3", "scenario": "S2"}, {"value": "0", "module": "C4"}, {"value": "-0.00396", "module": "D", "scenario": "S1"}, {"value": "-0.00123", "module": "D", "scenario": "S2"}]}}, {"referenceToLCIAMethodDataSet": {"shortDescription": [{"value": "Eutrophication potential aquatic freshwater (EP-freshwater)", "lang": "en"}, {"value": "Eutrophierungspotenzial Süßwasser (EP-freshwater)", "lang": "de"}], "type": "LCIA method data set", "refObjectId": "b53ec18f-7377-4ad3-86eb-cc3f4f276b2b", "uri": "../lciamethods/b53ec18f-7377-4ad3-86eb-cc3f4f276b2b.xml"}, "other": {"anies": [{"name": "referenceToUnitGroupDataSet", "value": {"shortDescription": [{"value": "kg PO_(4)-Äq.", "lang": "en"}], "type": "unit group data set", "refObjectId": "0429039d-a61d-4590-ba67-aa4a20a810a1", "uri": "../unitgroups/0429039d-a61d-4590-ba67-aa4a20a810a1.xml"}}, {"value": "3.13636363636364E-05", "module": "A1-A3"}, {"value": "4.78181818181818E-08", "module": "A4"}, {"value": "3.18664545454545E-06", "module": "A5"}, {"value": "0", "module": "C1"}, {"value": "4.54E-07", "module": "C2", "scenario": "S1"}, {"value": "1.83E-07", "module": "C2", "scenario": "S2"}, {"value": "3.39E-07", "module": "C3", "scenario": "S1"}, {"value": "1.03E-06", "module": "C3", "scenario": "S2"}, {"value": "0", "module": "C4"}, {"value": "-6.36E-06", "module": "D", "scenario": "S1"}, {"value": "-2.86E-06", "module": "D", "scenario": "S2"}]}}, {"referenceToLCIAMethodDataSet": {"shortDescription": [{"value": "Eutrophication potential aquatic marine (EP-marine)", "lang": "en"}, {"value": "Eutrophierungspotenzial Salzwasser (EP-marine)", "lang": "de"}], "type": "LCIA method data set", "refObjectId": "b5c619fa-def3-11e6-bf01-fe55135034f3", "uri": "../lciamethods/b5c619fa-def3-11e6-bf01-fe55135034f3.xml"}, "other": {"anies": [{"name": "referenceToUnitGroupDataSet", "value": {"shortDescription": [{"value": "kg N-Äq.", "lang": "en"}], "type": "unit group data set", "refObjectId": "d05bb823-ecdf-4686-8c40-bf1d9257859f", "uri": "../unitgroups/d05bb823-ecdf-4686-8c40-bf1d9257859f.xml"}}, {"value": "0.00206363636363636", "module": "A1-A3"}, {"value": "0.00035", "module": "A4"}, {"value": "0.000262563636363636", "module": "A5"}, {"value": "0", "module": "C1"}, {"value": "5.24E-05", "module": "C2", "scenario": "S1"}, {"value": "7.1E-06", "module": "C2", "scenario": "S2"}, {"value": "6.68E-05", "module": "C3", "scenario": "S1"}, {"value": "0.000363", "module": "C3", "scenario": "S2"}, {"value": "0", "module": "C4"}, {"value": "-0.00126", "module": "D", "scenario": "S1"}, {"value": "-0.000439", "module": "D", "scenario": "S2"}]}}, {"referenceToLCIAMethodDataSet": {"shortDescription": [{"value": "Eutrophication potential terrestrial (EP-terrestrial)", "lang": "en"}, {"value": "Eutrophierungspotenzial Land (EP-terrestrial)", "lang": "de"}], "type": "LCIA method data set", "refObjectId": "b5c614d2-def3-11e6-bf01-fe55135034f3", "uri": "../lciamethods/b5c614d2-def3-11e6-bf01-fe55135034f3.xml"}, "other": {"anies": [{"name": "referenceToUnitGroupDataSet", "value": {"shortDescription": [{"value": "mol N-Äq.", "lang": "en"}], "type": "unit group data set", "refObjectId": "71b4d617-0ec9-4d3f-b65e-e438940c2401", "uri": "../unitgroups/71b4d617-0ec9-4d3f-b65e-e438940c2401.xml"}}, {"value": "0.0212727272727273", "module": "A1-A3"}, {"value": "0.00383636363636364", "module": "A4"}, {"value": "0.00278090909090909", "module": "A5"}, {"value": "0", "module": "C1"}, {"value": "0.000616", "module": "C2", "scenario": "S1"}, {"value": "9.46E-05", "module": "C2", "scenario": "S2"}, {"value": "0.000724", "module": "C3", "scenario": "S1"}, {"value": "0.00451", "module": "C3", "scenario": "S2"}, {"value": "0", "module": "C4"}, {"value": "-0.0139", "module": "D", "scenario": "S1"}, {"value": "-0.00466", "module": "D", "scenario": "S2"}]}}, {"referenceToLCIAMethodDataSet": {"shortDescription": [{"value": "Formation potential of tropospheric ozone photochemical oxidants (POCP)", "lang": "en"}, {"value": "Bildungspotential für troposphärisches Ozon (POCP)", "lang": "de"}], "type": "LCIA method data set", "refObjectId": "b5c610fe-def3-11e6-bf01-fe55135034f3", "uri": "../lciamethods/b5c610fe-def3-11e6-bf01-fe55135034f3.xml"}, "other": {"anies": [{"name": "referenceToUnitGroupDataSet", "value": {"shortDescription": [{"value": "kg NMVOC-Äq.", "lang": "en"}], "type": "unit group data set", "refObjectId": "d27c25f8-fbc1-44c6-b47b-4adbae4199c6", "uri": "../unitgroups/d27c25f8-fbc1-44c6-b47b-4adbae4199c6.xml"}}, {"value": "0.0134545454545455", "module": "A1-A3"}, {"value": "0.000981818181818182", "module": "A4"}, {"value": "0.00150193636363636", "module": "A5"}, {"value": "0", "module": "C1"}, {"value": "0.000168", "module": "C2", "scenario": "S1"}, {"value": "2.82E-05", "module": "C2", "scenario": "S2"}, {"value": "0.000162", "module": "C3", "scenario": "S1"}, {"value": "0.00104", "module": "C3", "scenario": "S2"}, {"value": "0", "module": "C4"}, {"value": "-0.00699", "module": "D", "scenario": "S1"}, {"value": "-0.00113", "module": "D", "scenario": "S2"}]}}, {"referenceToLCIAMethodDataSet": {"shortDescription": [{"value": "Abiotic depletion potential for non fossil resources (ADPE)", "lang": "en"}, {"value": "Potenzial für den abiotischen Abbau nicht fossiler Ressourcen (ADPE)", "lang": "de"}], "type": "LCIA method data set", "refObjectId": "b2ad6494-c78d-11e6-9d9d-cec0c932ce01", "uri": "../lciamethods/b2ad6494-c78d-11e6-9d9d-cec0c932ce01.xml"}, "other": {"anies": [{"name": "referenceToUnitGroupDataSet", "value": {"shortDescription": [{"value": "kg Sb-Äq.", "lang": "en"}], "type": "unit group data set", "refObjectId": "54ccd2d9-a32a-4fc2-923d-f2c8c93e89d4", "uri": "../unitgroups/54ccd2d9-a32a-4fc2-923d-f2c8c93e89d4.xml"}}, {"value": "98.1818181818182", "module": "A1-A3"}, {"value": "0.685454545454545", "module": "A4"}, {"value": "10.2037272727273", "module": "A5"}, {"value": "0", "module": "C1"}, {"value": "2.07", "module": "C2", "scenario": "S1"}, {"value": "0.818", "module": "C2", "scenario": "S2"}, {"value": "0.999", "module": "C3", "scenario": "S1"}, {"value": "7.48", "module": "C3", "scenario": "S2"}, {"value": "0", "module": "C4"}, {"value": "-68.6", "module": "D", "scenario": "S1"}, {"value": "-16.9", "module": "D", "scenario": "S2"}]}}, {"referenceToLCIAMethodDataSet": {"shortDescription": [{"value": "Abiotic depletion potential for fossil resources (ADPF)", "lang": "en"}, {"value": "Potenzial für den abiotischen Abbau fossiler Brennstoffe (ADPF)", "lang": "de"}], "type": "LCIA method data set", "refObjectId": "b2ad6110-c78d-11e6-9d9d-cec0c932ce01", "uri": "../lciamethods/b2ad6110-c78d-11e6-9d9d-cec0c932ce01.xml"}, "other": {"anies": [{"name": "referenceToUnitGroupDataSet", "value": {"shortDescription": [{"value": "MJ", "lang": "en"}], "type": "unit group data set", "refObjectId": "93a60a57-a3c8-11da-a746-0800200c9a66", "uri": "../unitgroups/93a60a57-a3c8-11da-a746-0800200c9a66.xml"}}, {"value": "0.0625454545454545", "module": "A1-A3"}, {"value": "3.29090909090909E-09", "module": "A4"}, {"value": "0.00625454998363636", "module": "A5"}, {"value": "0", "module": "C1"}, {"value": "1.28E-08", "module": "C2", "scenario": "S1"}, {"value": "5.12E-09", "module": "C2", "scenario": "S2"}, {"value": "3.47E-08", "module": "C3", "scenario": "S1"}, {"value": "9.89E-08", "module": "C3", "scenario": "S2"}, {"value": "0", "module": "C4"}, {"value": "-5.55E-07", "module": "D", "scenario": "S1"}, {"value": "-3.24E-07", "module": "D", "scenario": "S2"}]}}, {"referenceToLCIAMethodDataSet": {"shortDescription": [{"value": "Water use (WDP)", "lang": "en"}, {"value": "Wassernutzung (WDP)", "lang": "de"}], "type": "LCIA method data set", "refObjectId": "b2ad66ce-c78d-11e6-9d9d-cec0c932ce01", "uri": "../lciamethods/b2ad66ce-c78d-11e6-9d9d-cec0c932ce01.xml"}, "other": {"anies": [{"name": "referenceToUnitGroupDataSet", "value": {"shortDescription": [{"value": "m^(3) world-Äq. deprived", "lang": "en"}], "type": "unit group data set", "refObjectId": "6ae2df01-888e-46c8-b17d-49fa3869b476", "uri": "../unitgroups/6ae2df01-888e-46c8-b17d-49fa3869b476.xml"}}, {"value": "0.359090909090909", "module": "A1-A3"}, {"value": "0.00014", "module": "A4"}, {"value": "0.0632230909090909", "module": "A5"}, {"value": "0", "module": "C1"}, {"value": "0.00137", "module": "C2", "scenario": "S1"}, {"value": "0.000549", "module": "C2", "scenario": "S2"}, {"value": "0.0145", "module": "C3", "scenario": "S1"}, {"value": "0.325", "module": "C3", "scenario": "S2"}, {"value": "0", "module": "C4"}, {"value": "-0.109", "module": "D", "scenario": "S1"}, {"value": "-0.0162", "module": "D", "scenario": "S2"}]}}, {"referenceToLCIAMethodDataSet": {"shortDescription": [{"value": "Incidence of disease due to PM emissions (PM)", "lang": "en"}, {"value": "Auftreten von Krankheiten aufgrund von Feinstaubemissionen (PM)", "lang": "de"}], "type": "LCIA method data set", "refObjectId": "b5c602c6-def3-11e6-bf01-fe55135034f3", "uri": "../lciamethods/b5c602c6-def3-11e6-bf01-fe55135034f3.xml"}, "other": {"anies": [{"name": "referenceToUnitGroupDataSet", "value": {"shortDescription": [{"value": "Disease incidence", "lang": "en"}], "type": "unit group data set", "refObjectId": "3883559b-648f-4afc-8ba2-0bd24f3affa3", "uri": "../unitgroups/3883559b-648f-4afc-8ba2-0bd24f3affa3.xml"}}, {"value": "47.1818181818182", "module": "A1-A3"}, {"value": "0.500909090909091", "module": "A4"}, {"value": "4.96527272727273", "module": "A5"}, {"value": "0", "module": "C1"}, {"value": "1.44", "module": "C2", "scenario": "S1"}, {"value": "0.568", "module": "C2", "scenario": "S2"}, {"value": "0.399", "module": "C3", "scenario": "S1"}, {"value": "6.29", "module": "C3", "scenario": "S2"}, {"value": "0", "module": "C4"}, {"value": "-34.7", "module": "D", "scenario": "S1"}, {"value": "-3.25", "module": "D", "scenario": "S2"}]}}, {"referenceToLCIAMethodDataSet": {"shortDescription": [{"value": "Human exposure efficiency relative to U235 (IR)", "lang": "en"}, {"value": "Wirkung durch Exposition des Menschen mit U235 (IR)", "lang": "de"}], "type": "LCIA method data set", "refObjectId": "b5c632be-def3-11e6-bf01-fe55135034f3", "uri": "../lciamethods/b5c632be-def3-11e6-bf01-fe55135034f3.xml"}, "other": {"anies": [{"name": "referenceToUnitGroupDataSet", "value": {"shortDescription": [{"value": "kBq U235-Äq.", "lang": "en"}], "type": "unit group data set", "refObjectId": "456b05bf-1415-44a9-9993-02452f554c09", "uri": "../unitgroups/456b05bf-1415-44a9-9993-02452f554c09.xml"}}, {"value": "1.94545454545455E-09", "module": "A1-A3"}, {"value": "9.54545454545454E-12", "module": "A4"}, {"value": "2.0308E-10", "module": "A5"}, {"value": "0", "module": "C1"}, {"value": "2.89E-11", "module": "C2", "scenario": "S1"}, {"value": "1.14E-11", "module": "C2", "scenario": "S2"}, {"value": "1.6E-11", "module": "C3", "scenario": "S1"}, {"value": "2.5E-10", "module": "C3", "scenario": "S2"}, {"value": "0", "module": "C4"}, {"value": "-9.64E-10", "module": "D", "scenario": "S1"}, {"value": "-1.87E-10", "module": "D", "scenario": "S2"}]}}, {"referenceToLCIAMethodDataSet": {"shortDescription": [{"value": "Comparative toxic unit for ecosystems (ETP-fw)", "lang": "en"}, {"value": "Toxizitätsvergleichseinheit für Ökosysteme (ETP-fw)", "lang": "de"}], "type": "LCIA method data set", "refObjectId": "ee1082d1-b0f7-43ca-a1f0-21e2a4a74511", "uri": "../lciamethods/ee1082d1-b0f7-43ca-a1f0-21e2a4a74511.xml"}, "other": {"anies": [{"name": "referenceToUnitGroupDataSet", "value": {"shortDescription": [{"value": "CTUe", "lang": "en"}], "type": "unit group data set", "refObjectId": "aa959ded-f1eb-4efb-9c5c-2d60be36b3e6", "uri": "../unitgroups/aa959ded-f1eb-4efb-9c5c-2d60be36b3e6.xml"}}, {"value": "3.51818181818182E-07", "module": "A1-A3"}, {"value": "4.57272727272727E-10", "module": "A4"}, {"value": "3.58325454545455E-08", "module": "A5"}, {"value": "0", "module": "C1"}, {"value": "1.47E-09", "module": "C2", "scenario": "S1"}, {"value": "5.83E-10", "module": "C2", "scenario": "S2"}, {"value": "7.4E-10", "module": "C3", "scenario": "S1"}, {"value": "2.67E-08", "module": "C3", "scenario": "S2"}, {"value": "0", "module": "C4"}, {"value": "-3.68E-08", "module": "D", "scenario": "S1"}, {"value": "-8.29E-09", "module": "D", "scenario": "S2"}]}}, {"referenceToLCIAMethodDataSet": {"shortDescription": [{"value": "Comparative toxic unit for humans (carcinogenic) (HTP-c)", "lang": "en"}, {"value": "Toxizitätsvergleichseinheit für Menschen (krebserregend) (HTP-c)", "lang": "de"}], "type": "LCIA method data set", "refObjectId": "2299222a-bbd8-474f-9d4f-4dd1f18aea7c", "uri": "../lciamethods/2299222a-bbd8-474f-9d4f-4dd1f18aea7c.xml"}, "other": {"anies": [{"name": "referenceToUnitGroupDataSet", "value": {"shortDescription": [{"value": "CTUh", "lang": "en"}], "type": "unit group data set", "refObjectId": "d4c9523e-2d7e-49fd-8469-998f547d3a70", "uri": "../unitgroups/d4c9523e-2d7e-49fd-8469-998f547d3a70.xml"}}, {"value": "26.5454545454545", "module": "A1-A3"}, {"value": "0.0818181818181818", "module": "A4"}, {"value": "2.75582727272727", "module": "A5"}, {"value": "0", "module": "C1"}, {"value": "0.698", "module": "C2", "scenario": "S1"}, {"value": "0.281", "module": "C2", "scenario": "S2"}, {"value": "0.526", "module": "C3", "scenario": "S1"}, {"value": "1.72", "module": "C3", "scenario": "S2"}, {"value": "0", "module": "C4"}, {"value": "-6.57", "module": "D", "scenario": "S1"}, {"value": "-4.43", "module": "D", "scenario": "S2"}]}}, {"referenceToLCIAMethodDataSet": {"shortDescription": [{"value": "Comparative toxic unit for humans (noncarcinogenic) (HTP-nc)", "lang": "en"}, {"value": "Toxizitätsvergleichseinheit für Menschen (nicht krebserregend) (HTP-nc)", "lang": "de"}], "type": "LCIA method data set", "refObjectId": "3af763a5-b7a1-48c9-9cee-1f223481fcef", "uri": "../lciamethods/3af763a5-b7a1-48c9-9cee-1f223481fcef.xml"}, "other": {"anies": [{"name": "referenceToUnitGroupDataSet", "value": {"shortDescription": [{"value": "CTUh", "lang": "en"}], "type": "unit group data set", "refObjectId": "d4c9523e-2d7e-49fd-8469-998f547d3a70", "uri": "../unitgroups/d4c9523e-2d7e-49fd-8469-998f547d3a70.xml"}}, {"value": "0", "module": "A1-A3"}, {"value": "0", "module": "A4"}, {"value": "0", "module": "A5"}, {"value": "0", "module": "C1"}, {"value": "0", "module": "C2", "scenario": "S1"}, {"value": "0", "module": "C2", "scenario": "S2"}, {"value": "0", "module": "C3", "scenario": "S1"}, {"value": "0", "module": "C3", "scenario": "S2"}, {"value": "0", "module": "C4"}, {"value": "0", "module": "D", "scenario": "S1"}, {"value": "0", "module": "D", "scenario": "S2"}]}}, {"referenceToLCIAMethodDataSet": {"shortDescription": [{"value": "Soil quality index (SQP)", "lang": "en"}, {"value": "Bodenqualitätsindex (SQP)", "lang": "de"}], "type": "LCIA method data set", "refObjectId": "b2ad6890-c78d-11e6-9d9d-cec0c932ce01", "uri": "../lciamethods/b2ad6890-c78d-11e6-9d9d-cec0c932ce01.xml"}, "other": {"anies": [{"name": "referenceToUnitGroupDataSet", "value": {"shortDescription": [{"value": "SQP", "lang": "en"}], "type": "unit group data set", "refObjectId": "f130951c-e67f-4f7f-8dd4-665de3974e18", "uri": "../unitgroups/f130951c-e67f-4f7f-8dd4-665de3974e18.xml"}}, {"value": "0", "module": "A1-A3"}, {"value": "0", "module": "A4"}, {"value": "0", "module": "A5"}, {"value": "0", "module": "C1"}, {"value": "0", "module": "C2", "scenario": "S1"}, {"value": "0", "module": "C2", "scenario": "S2"}, {"value": "0", "module": "C3", "scenario": "S1"}, {"value": "0", "module": "C3", "scenario": "S2"}, {"value": "0", "module": "C4"}, {"value": "0", "module": "D", "scenario": "S1"}, {"value": "0", "module": "D", "scenario": "S2"}]}}]}, "otherAttributes": {"{http://www.indata.network/EPD/2019}epd-version": "1.2"}, "version": "1.1", "locations": "../ILCDLocations.xml"}