{"processInformation": {"dataSetInformation": {"UUID": "b5928b77-fe98-4b04-994a-4baae5674c2e", "name": {"baseName": [{"value": "Lichtkuppeln - LAMILUX Heinrich Strunz GmbH - Rauchlift Lichtkuppel F100 RWA SAN (2025)", "lang": "de"}, {"value": "Rooflight domes - LAMILUX Heinrich Strunz GmbH - Smoke lift rooflight F100 RWA SAN (2025)", "lang": "en"}]}, "synonyms": [{"value": "Tageslichtsystem", "lang": "de"}, {"value": "Daylight system", "lang": "en"}], "classificationInformation": {"classification": [{"class": [{"value": "Komponenten von Fenstern und Vorhangfassaden", "level": 0, "classId": "7"}, {"value": "Tageslichtsysteme und Rauch- / Wärmeabzugsanlagen ", "level": 1, "classId": "7.10"}, {"value": "Rauch-/Wärmeabzugsanlagen", "level": 2, "classId": "7.10.02"}], "name": "OEKOBAU.DAT"}]}, "generalComment": [{"value": "Dieser Datensatz beinhaltet die Ergebnisse für die Module A1-A3 sowie Module A4, A5, B2, B3, B4, C1, C2, C3, C4, D. Das Umweltprofil beinhaltet die Aufwendungen für die Lebenszyklus-Stadien cradle to gate with options (Modul A1-A3). Die Herstellung der Verpackung wurde innerhalb der Module A1-A3 berücksichtigt.", "lang": "de"}, {"value": "This data set contains the results for modules A1-A3 and modules A4, A5, B2, B3, B4, C1, C2, C3, C4, D. The environmental profile includes the expenses for the life cycle stages cradle to gate with options (modules A1-A3). The production of the packaging was taken into account within modules A1-A3.", "lang": "en"}]}, "quantitativeReference": {"referenceToReferenceFlow": [1], "type": "Reference flow(s)"}, "time": {"referenceYear": 2025, "dataSetValidUntil": 2030, "timeRepresentativenessDescription": [{"value": "jährlicher Durchschnitt", "lang": "de"}, {"value": "annual average", "lang": "en"}], "other": {"anies": [{"name": "publicationDateOfEPD", "value": 1742774400000}]}}, "geography": {"locationOfOperationSupplyOrProduction": {"descriptionOfRestrictions": [{"value": "Dieser Datensatz repräsentiert die Situation des Unternehmens LAMILUX Heinrich Strunz GmbH, 95111 Rehau im Hinblick auf die wichtigsten Technologien und die gesetzlichen Rahmenbedingungen.", "lang": "de"}, {"value": "This data set represents the situation of the company LAMILUX Heinrich Strunz GmbH, 95111 Rehau with regard to the most important technologies and the legal framework.", "lang": "en"}], "location": "DE"}}, "technology": {"technologyDescriptionAndIncludedProcesses": [{"value": "Die Ökobilanzergebnisse umfassen die Lebenszyklusstadien der Herstellung der Vorprodukte bis hin zur Rohstoffgewinnung und Verarbeitungsprozesse von als Input dienenden Sekundärstoffen (z.B. Recyclingprozesse), deren Transporte zum Werk sowie die Produktion selbst, einschließlich der Bereitstellung von allen Hilfs- und Betriebsstoffen, Energie, sowie die vollständige Abfallbehandlung oder die Deponierung der Restabfälle während des Stadiums der Produktion. Die Module A1, A2 und A3 sind hier als ein aggregiertes Modul A1-A3 ausgewiesen. Falls für diesen Datensatz weitere Module berechnet wurden, sind diese separat zu finden und können für eine Betrachtung des gesamten Lebenszyklus zusammengeführt werden.", "lang": "de"}, {"value": "The life cycle assessment results cover the life cycle stages from the manufacture of primary products to the extraction of raw materials and processing of secondary materials used as input (e.g. recycling processes), their transportation to the plant and the production itself, including the provision of all auxiliary and operating materials, energy, as well as the complete waste treatment or landfilling of residual waste during the production stage. Modules A1, A2 and A3 are shown here as an aggregated module A1-A3. If further modules were calculated for this data set, these can be found separately and can be combined for a consideration of the entire life cycle.", "lang": "en"}], "technologicalApplicability": [{"value": "Tageslichtsysteme zur Erhöhung des Tageslichteinfalls, zur natürlichen Be-und Entlüftung und zum Rauch- und Wärmeabzug.\r\nMultifunktionale Tageslichtsysteme und Glasdachkonstruktionen kommen zur Anwendung z.B. in:\r\nBüro- und Verwaltungsgebäuden; Industriegebäuden; Öffentlichen Gebäuden; Privaten Gebäuden.\r\n", "lang": "de"}, {"value": "Daylight systems to increase daylight intake, for natural ventilation and smoke and heat extraction.\r\nMultifunctional daylight systems and glass roof constructions are used in e.g:\r\nOffice and administration buildings; Industrial buildings; Public buildings; Private buildings.", "lang": "en"}]}}, "modellingAndValidation": {"LCIMethodAndAllocation": {"typeOfDataSet": "EPD", "referenceToLCAMethodDetails": [{"shortDescription": [{"value": "Produktkategorieregeln Teil A", "lang": "de"}], "type": "source data set", "refObjectId": "c6e986be-62a9-4f2f-b486-27aa9129eaeb", "version": "00.00.006"}, {"shortDescription": [{"value": "Produktkategorieregeln Teil B – für Fenster, Flachdachfenster, Lichtkuppeln und Lichtbänder", "lang": "de"}], "type": "source data set", "refObjectId": "8d6b7091-7bcc-4436-a2c1-98dd9aa19d6e", "version": "00.00.003"}], "other": {"anies": [{"name": "subType", "value": "specific dataset"}]}}, "dataSourcesTreatmentAndRepresentativeness": {"referenceToDataSource": [{"shortDescription": [{"value": "ecoinvent database (general)", "lang": "en"}], "type": "source data set", "refObjectId": "b497a91f-e14b-4b69-8f28-f50eb1576766", "version": "00.03.002"}], "useAdviceForDataSet": [{"value": "Dieser Datensatz beinhaltet die Ergebnisse für die Module A1-A3 sowie die Module A4, A5, B2, B3, B4, C1, C2, C3, C4 und D gemäß EN 15804 + A2.\r\nDie Modellierung der B-Module wurde bezogen auf 1 Jahr vorgenommen.\r\nEin Vergleich mit anderen Produkten ist nur mit einer vergleichbaren Anwendung im Gebäude zulässig. Grundsätzlich ist eine Gegenüberstellung oder die Bewertung von EPD Daten nur möglich, wenn alle zu vergleichenden Datensätze nach EN 15804 + A2 erstellt wurden und der Gebäudekontext, bzw. die produktspezifischen Leistungsmerkmale berücksichtigt werden.", "lang": "de"}, {"value": "This data set contains the results for modules A1-A3 as well as modules A4, A5, B2, B3, B4, C1, C2, C3, C4 and D in accordance with EN 15804 + A2.\r\nThe modelling of the B modules was carried out in relation to 1 year.\r\nA comparison with other products is only permissible with a comparable application in the building. In principle, a comparison or evaluation of EPD data is only possible if all data sets to be compared were created in accordance with EN 15804 + A2 and the building context or the product-specific performance characteristics are taken into account.", "lang": "en"}], "other": {"anies": [{"name": "referenceToOriginalEPD", "value": {"shortDescription": {"value": "EPD - Lichtkuppeln - LAMILUX - Rauchlift Lichtkuppel F100", "defaultValue": "EPD - Lichtkuppeln - LAMILUX - Rauchlift Lichtkuppel F100", "lstrings": [{"lang": "de", "value": "EPD - Lichtkuppeln - LAMILUX - Rauchlift Lichtkuppel F100"}]}, "version": {"version": 1, "majorVersion": 0, "minorVersion": 0, "subMinorVersion": 1, "zero": false, "versionString": "00.00.001"}, "type": "source data set", "uuid": {"uuid": "5c3e126a-30c5-417c-ad89-fc8befba9229"}, "refObjectId": "5c3e126a-30c5-417c-ad89-fc8befba9229", "versionAsString": "00.00.001", "resourceURLs": ["https://oekobaudat.de/OEKOBAU.DAT/resource/sources/5c3e126a-30c5-417c-ad89-fc8befba9229/EPD-RLK-GB-11.5.pdf?version=00.00.001", "https://oekobaudat.de/OEKOBAU.DAT/resource/sources/5c3e126a-30c5-417c-ad89-fc8befba9229/EPD-RLK-11.5.pdf?version=00.00.001"]}}]}}, "validation": {"review": [{"reviewDetails": [{"value": "Die angewendete LCI Methode ist in Übereinstimmung mit ISO 14040 und 14044. Die Dokumentation enthält alle relevanten Informationen im Hinblick auf die Datenqualität und den Umfang der Anwendung der jeweiligen LCI Ergebnisse bzw. der Datensätze. Der Datensatz repräsentiert den Stand der Technik bezogen auf die funktionelle Einheit.", "lang": "de"}, {"value": "The LCI method used is in accordance with ISO 14040 and 14044. The documentation contains all relevant information with regard to the data quality and the scope of application of the respective LCI results or data sets. The data set represents the state of the art in relation to the functional unit.", "lang": "en"}], "referenceToNameOfReviewerAndInstitution": [{"shortDescription": [{"value": "Susanne Volz", "lang": "de"}], "type": "contact data set", "refObjectId": "39da5078-3db5-40dd-bcc6-145b1dc8870d", "version": "00.00.002"}], "type": "Independent external review"}]}, "complianceDeclarations": {"compliance": [{"referenceToComplianceSystem": {"shortDescription": [{"value": "EN 15804+A2", "lang": "de"}, {"value": "EN 15804+A2", "lang": "en"}], "type": "source data set", "refObjectId": "c0016b33-8cf7-415c-ac6e-deba0d21440d", "version": "00.01.003"}}]}}, "administrativeInformation": {"dataGenerator": {"referenceToPersonOrEntityGeneratingTheDataSet": [{"shortDescription": [{"value": "LAMILUX Heinrich Strunz GmbH", "lang": "de"}], "type": "contact data set", "refObjectId": "534a2cc0-9495-4dec-8354-3d0bf18d1edc", "version": "00.00.002"}]}, "dataEntryBy": {"timeStamp": 1745395013076, "referenceToDataSetFormat": [{"shortDescription": [{"value": "EPD Data Format Extensions v1.2", "lang": "en"}, {"value": "EPD-Datenformaterweiterungen v1.2", "lang": "de"}], "type": "source data set", "refObjectId": "a29449fd-aa2f-4de8-b5d7-4b06b43c6fde", "version": "00.01.003"}, {"shortDescription": [{"value": "ILCD format", "lang": "en"}], "type": "source data set", "refObjectId": "a97a0155-0234-4b87-b4ce-a45da52f2a40", "version": "03.01.004", "uri": "http://lca.jrc.ec.europa.eu/lcainfohub/datasets/ilcd/sources/a97a0155-0234-4b87-b4ce-a45da52f2a40.xml"}], "referenceToPersonOrEntityEnteringTheData": {"shortDescription": [{"value": "ift Rosenheim", "lang": "de"}], "type": "contact data set", "refObjectId": "bdf65bd4-c474-4c23-8269-124ba43fa2b9", "version": "25.00.001"}}, "publicationAndOwnership": {"dataSetVersion": "00.00.030", "referenceToPrecedingDataSetVersion": [{"shortDescription": [{"value": "Lichtkuppeln - LAMILUX Heinrich Strunz GmbH - Rauchlift Lichtkuppel F100", "lang": "de"}], "type": "process data set", "refObjectId": "c727edab-e821-49e8-908f-6017a1713826", "version": "00.00.009"}], "referenceToRegistrationAuthority": {"shortDescription": [{"value": "ift Rosenheim", "lang": "de"}], "type": "contact data set", "refObjectId": "bdf65bd4-c474-4c23-8269-124ba43fa2b9", "version": "25.00.001"}, "registrationNumber": "EPD-RLK-11.5", "referenceToOwnershipOfDataSet": {"shortDescription": [{"value": "LAMILUX Heinrich Strunz GmbH", "lang": "de"}], "type": "contact data set", "refObjectId": "534a2cc0-9495-4dec-8354-3d0bf18d1edc", "version": "00.00.002"}, "copyright": true, "licenseType": "Free of charge for all users and uses", "accessRestrictions": [{"value": "none", "lang": "de"}, {"value": "none", "lang": "en"}], "other": {"anies": [{"name": "referenceToPublisher", "value": {"shortDescription": [{"value": "ift Rosenheim", "lang": "de"}], "type": "contact data set", "refObjectId": "bdf65bd4-c474-4c23-8269-124ba43fa2b9", "version": "25.00.001"}}]}}}, "exchanges": {"exchange": [{"dataSetInternalID": 1, "referenceToFlowDataSet": {"shortDescription": [{"value": "Lichtkuppeln - LAMILUX - Rauchlift Lichtkuppel F100 RWA SAN (2025)", "lang": "de"}, {"value": "Rooflight domes - LAMILUX - Smoke lift rooflight F100 RWA SAN (2025)", "lang": "en"}], "type": "flow data set", "refObjectId": "fb1f7df2-1132-4a76-82c6-61c13a18cae9", "version": "00.00.003"}, "meanAmount": 1.0, "resultingAmount": 1.0, "referenceFlow": true, "resultingflowAmount": 1.0, "flowProperties": [{"name": [{"lang": "de", "value": "Fläche"}, {"lang": "en", "value": "Area"}], "uuid": "93a60a56-a3c8-19da-a746-0800200c9a66", "referenceFlowProperty": true, "meanValue": 1.0, "referenceUnit": "qm", "unitGroupUUID": "c20a03d7-bd90-4569-bc94-66cfd364dfc8"}], "materialProperties": [{"name": "grammage", "value": "30.11", "unit": "kg/m^2", "unitDescription": "kilograms per square meter"}, {"name": "layer thickness", "value": "0.3", "unit": "m", "unitDescription": "meters"}], "typeOfFlow": "Product flow", "classification": {"classHierarchy": "Komponenten von Fenstern und Vorhangfassaden / Tageslichtsysteme und Rauch- / Wärmeabzugsanlagen / Rauch-/Wärmeabzugsanlagen", "name": "ilcd"}}, {"dataSetInternalID": 2, "referenceToFlowDataSet": {"shortDescription": [{"value": "Components for re-use (CRU)", "lang": "en"}, {"value": "Komponenten für die Wiederverwendung (CRU)", "lang": "de"}], "type": "flow data set", "refObjectId": "a2b32f97-3fc7-4af2-b209-525bc6426f33", "version": "38.00.000"}, "exchange direction": "OUTPUT", "meanAmount": 0.0, "other": {"anies": [{"value": "0.0", "module": "A1-A3"}, {"value": "0.0", "module": "A4"}, {"value": "0.0", "module": "A5"}, {"value": "0.0", "module": "B2"}, {"value": "0.0", "module": "B3"}, {"value": "0.0", "module": "B4"}, {"value": "0.0", "module": "C1"}, {"value": "0.0", "module": "C2"}, {"value": "0.0", "module": "C3"}, {"value": "0.0", "module": "C4"}, {"value": "0.0", "module": "D"}, {"name": "referenceToUnitGroupDataSet", "value": {"shortDescription": [{"value": "kg"}], "type": "unit group data set", "refObjectId": "ad38d542-3fe9-439d-9b95-2f5f7752acaf", "uri": "../unitgroups/ad38d542-3fe9-439d-9b95-2f5f7752acaf"}}]}, "flowProperties": [], "typeOfFlow": "Other flow", "classification": {"classHierarchy": "Quantities / Environmental quantities / EPD EN 15804 / LCI indicators", "name": "GaBiCategories"}}, {"dataSetInternalID": 3, "referenceToFlowDataSet": {"shortDescription": [{"value": "Exported electrical energy (EEE)", "lang": "en"}, {"value": "Exportierte elektrische Energie (EEE)", "lang": "de"}], "type": "flow data set", "refObjectId": "4da0c987-2b76-40d6-9e9e-82a017aaaf29", "version": "38.00.000"}, "exchange direction": "OUTPUT", "meanAmount": 0.0, "other": {"anies": [{"value": "4.86", "module": "A1-A3"}, {"value": "0.00536", "module": "A4"}, {"value": "0.329", "module": "A5"}, {"value": "4.75E-4", "module": "B2"}, {"value": "0.00265", "module": "B3"}, {"value": "5.35", "module": "B4"}, {"value": "0.0", "module": "C1"}, {"value": "3.42E-4", "module": "C2"}, {"value": "0.148", "module": "C3"}, {"value": "4.06E-4", "module": "C4"}, {"value": "-4.2", "module": "D"}, {"name": "referenceToUnitGroupDataSet", "value": {"shortDescription": [{"value": "MJ"}], "type": "unit group data set", "refObjectId": "93a60a57-a3c8-11da-a746-0800200c9a66", "uri": "../unitgroups/93a60a57-a3c8-11da-a746-0800200c9a66"}}]}, "flowProperties": [], "typeOfFlow": "Other flow", "classification": {"classHierarchy": "Quantities / Environmental quantities / EPD EN 15804 / LCI indicators", "name": "GaBiCategories"}}, {"dataSetInternalID": 4, "referenceToFlowDataSet": {"shortDescription": [{"value": "Exported thermal energy (EET)", "lang": "en"}, {"value": "Exportierte thermische Energie (EET)", "lang": "de"}], "type": "flow data set", "refObjectId": "98daf38a-7a79-46d3-9a37-2b7bd0955810", "version": "38.00.000"}, "exchange direction": "OUTPUT", "meanAmount": 0.0, "other": {"anies": [{"value": "4.99", "module": "A1-A3"}, {"value": "0.0268", "module": "A4"}, {"value": "0.013", "module": "A5"}, {"value": "0.00159", "module": "B2"}, {"value": "0.00384", "module": "B3"}, {"value": "5.06", "module": "B4"}, {"value": "0.0", "module": "C1"}, {"value": "4.1E-4", "module": "C2"}, {"value": "0.0121", "module": "C3"}, {"value": "0.00708", "module": "C4"}, {"value": "-0.68", "module": "D"}, {"name": "referenceToUnitGroupDataSet", "value": {"shortDescription": [{"value": "MJ"}], "type": "unit group data set", "refObjectId": "93a60a57-a3c8-11da-a746-0800200c9a66", "uri": "../unitgroups/93a60a57-a3c8-11da-a746-0800200c9a66"}}]}, "flowProperties": [], "typeOfFlow": "Other flow", "classification": {"classHierarchy": "Quantities / Environmental quantities / EPD EN 15804 / LCI indicators", "name": "GaBiCategories"}}, {"dataSetInternalID": 5, "referenceToFlowDataSet": {"shortDescription": [{"value": "Hazardous waste disposed (HWD)", "lang": "en"}, {"value": "Gefährlicher Abfall zur Beseitigung (HWD)", "lang": "de"}], "type": "flow data set", "refObjectId": "430f9e0f-59b2-46a0-8e0d-55e0e84948fc", "version": "38.00.000"}, "exchange direction": "OUTPUT", "meanAmount": 0.0, "other": {"anies": [{"value": "47.8", "module": "A1-A3"}, {"value": "0.0245", "module": "A4"}, {"value": "0.058", "module": "A5"}, {"value": "0.00248", "module": "B2"}, {"value": "0.118", "module": "B3"}, {"value": "49.2", "module": "B4"}, {"value": "0.0", "module": "C1"}, {"value": "0.00229", "module": "C2"}, {"value": "1.12", "module": "C3"}, {"value": "0.00179", "module": "C4"}, {"value": "-27.6", "module": "D"}, {"name": "referenceToUnitGroupDataSet", "value": {"shortDescription": [{"value": "kg"}], "type": "unit group data set", "refObjectId": "ad38d542-3fe9-439d-9b95-2f5f7752acaf", "uri": "../unitgroups/ad38d542-3fe9-439d-9b95-2f5f7752acaf"}}]}, "flowProperties": [], "typeOfFlow": "Other flow", "classification": {"classHierarchy": "Quantities / Environmental quantities / EPD EN 15804 / LCI indicators", "name": "GaBiCategories"}}, {"dataSetInternalID": 6, "referenceToFlowDataSet": {"shortDescription": [{"value": "Material for Energy Recovery (MER)", "lang": "en"}, {"value": "Stoff für die Energierückgewinnung (MER)", "lang": "de"}], "type": "flow data set", "refObjectId": "59a9181c-3aaf-46ee-8b13-2b3723b6e447", "version": "38.00.000"}, "exchange direction": "OUTPUT", "meanAmount": 0.0, "other": {"anies": [{"value": "0.00178", "module": "A1-A3"}, {"value": "4.65E-6", "module": "A4"}, {"value": "3.9E-6", "module": "A5"}, {"value": "3.71E-7", "module": "B2"}, {"value": "2.19E-6", "module": "B3"}, {"value": "0.00182", "module": "B4"}, {"value": "0.0", "module": "C1"}, {"value": "2.74E-7", "module": "C2"}, {"value": "2.87E-5", "module": "C3"}, {"value": "3.79E-7", "module": "C4"}, {"value": "-2.21E-4", "module": "D"}, {"name": "referenceToUnitGroupDataSet", "value": {"shortDescription": [{"value": "kg"}], "type": "unit group data set", "refObjectId": "ad38d542-3fe9-439d-9b95-2f5f7752acaf", "uri": "../unitgroups/ad38d542-3fe9-439d-9b95-2f5f7752acaf"}}]}, "flowProperties": [], "typeOfFlow": "Other flow", "classification": {"classHierarchy": "Quantities / Environmental quantities / EPD EN 15804 / LCI indicators", "name": "GaBiCategories"}}, {"dataSetInternalID": 7, "referenceToFlowDataSet": {"shortDescription": [{"value": "Materials for Recycling (MFR)", "lang": "en"}, {"value": "Stoffe zum Recycling (MFR)", "lang": "de"}], "type": "flow data set", "refObjectId": "d7fe48a5-4103-49c8-9aae-b0b5dfdbd6ae", "version": "38.00.000"}, "exchange direction": "OUTPUT", "meanAmount": 0.0, "other": {"anies": [{"value": "9.14", "module": "A1-A3"}, {"value": "0.0294", "module": "A4"}, {"value": "0.025", "module": "A5"}, {"value": "0.00286", "module": "B2"}, {"value": "0.0141", "module": "B3"}, {"value": "9.6", "module": "B4"}, {"value": "0.0", "module": "C1"}, {"value": "0.00207", "module": "C2"}, {"value": "0.336", "module": "C3"}, {"value": "0.00189", "module": "C4"}, {"value": "-0.995", "module": "D"}, {"name": "referenceToUnitGroupDataSet", "value": {"shortDescription": [{"value": "kg"}], "type": "unit group data set", "refObjectId": "ad38d542-3fe9-439d-9b95-2f5f7752acaf", "uri": "../unitgroups/ad38d542-3fe9-439d-9b95-2f5f7752acaf"}}]}, "flowProperties": [], "typeOfFlow": "Other flow", "classification": {"classHierarchy": "Quantities / Environmental quantities / EPD EN 15804 / LCI indicators", "name": "GaBiCategories"}}, {"dataSetInternalID": 8, "referenceToFlowDataSet": {"shortDescription": [{"value": "Use of net fresh water (FW)", "lang": "en"}, {"value": "Frischwasserverbrauch (FW)", "lang": "de"}], "type": "flow data set", "refObjectId": "3cf952c8-f3a4-461d-8c96-96456ca62246", "version": "38.00.000"}, "exchange direction": "INPUT", "meanAmount": 0.0, "other": {"anies": [{"value": "1.5", "module": "A1-A3"}, {"value": "0.00362", "module": "A4"}, {"value": "0.0167", "module": "A5"}, {"value": "0.00113", "module": "B2"}, {"value": "0.00233", "module": "B3"}, {"value": "1.7", "module": "B4"}, {"value": "0.0", "module": "C1"}, {"value": "3.35E-4", "module": "C2"}, {"value": "0.193", "module": "C3"}, {"value": "-0.0242", "module": "C4"}, {"value": "-0.425", "module": "D"}, {"name": "referenceToUnitGroupDataSet", "value": {"shortDescription": [{"value": "m3"}], "type": "unit group data set", "refObjectId": "cd950537-0a98-4044-9ba7-9f9a68d0a504", "uri": "../unitgroups/cd950537-0a98-4044-9ba7-9f9a68d0a504"}}]}, "flowProperties": [], "typeOfFlow": "Other flow", "classification": {"classHierarchy": "Quantities / Environmental quantities / EPD EN 15804 / LCI indicators", "name": "GaBiCategories"}}, {"dataSetInternalID": 9, "referenceToFlowDataSet": {"shortDescription": [{"value": "Non-hazardous waste disposed (NHWD)", "lang": "en"}, {"value": "Ungefährlicher Abfall zur Beseitigung (NHWD)", "lang": "de"}], "type": "flow data set", "refObjectId": "b29ef66b-e286-4afa-949f-62f1a7b4d7fa", "version": "38.00.000"}, "exchange direction": "OUTPUT", "meanAmount": 0.0, "other": {"anies": [{"value": "204.0", "module": "A1-A3"}, {"value": "0.297", "module": "A4"}, {"value": "8.56", "module": "A5"}, {"value": "0.29", "module": "B2"}, {"value": "0.436", "module": "B3"}, {"value": "270.0", "module": "B4"}, {"value": "0.0", "module": "C1"}, {"value": "0.0222", "module": "C2"}, {"value": "24.7", "module": "C3"}, {"value": "31.6", "module": "C4"}, {"value": "-19.4", "module": "D"}, {"name": "referenceToUnitGroupDataSet", "value": {"shortDescription": [{"value": "kg"}], "type": "unit group data set", "refObjectId": "ad38d542-3fe9-439d-9b95-2f5f7752acaf", "uri": "../unitgroups/ad38d542-3fe9-439d-9b95-2f5f7752acaf"}}]}, "flowProperties": [], "typeOfFlow": "Other flow", "classification": {"classHierarchy": "Quantities / Environmental quantities / EPD EN 15804 / LCI indicators", "name": "GaBiCategories"}}, {"dataSetInternalID": 10, "referenceToFlowDataSet": {"shortDescription": [{"value": "Nicht-erneuerbare Primärenergie als Energieträger (PENRE)", "lang": "en"}, {"value": "Nicht-erneuerbare Primärenergie als Energieträger (PENRE)", "lang": "de"}], "type": "flow data set", "refObjectId": "ac857178-2b45-46ec-892a-a9a4332f0372", "version": "38.00.000"}, "exchange direction": "INPUT", "meanAmount": 0.0, "other": {"anies": [{"value": "2500.0", "module": "A1-A3"}, {"value": "21.6", "module": "A4"}, {"value": "22.8", "module": "A5"}, {"value": "1.1", "module": "B2"}, {"value": "2.23", "module": "B3"}, {"value": "2630.0", "module": "B4"}, {"value": "0.0", "module": "C1"}, {"value": "2.09", "module": "C2"}, {"value": "28.3", "module": "C3"}, {"value": "1.47", "module": "C4"}, {"value": "-569.0", "module": "D"}, {"name": "referenceToUnitGroupDataSet", "value": {"shortDescription": [{"value": "MJ"}], "type": "unit group data set", "refObjectId": "93a60a57-a3c8-11da-a746-0800200c9a66", "uri": "../unitgroups/93a60a57-a3c8-11da-a746-0800200c9a66"}}]}, "flowProperties": [], "typeOfFlow": "Other flow", "classification": {"classHierarchy": "Quantities", "name": "GaBiCategories"}}, {"dataSetInternalID": 11, "referenceToFlowDataSet": {"shortDescription": [{"value": "Nicht-erneuerbare Primärenergie zur stofflichen Nutzung (PENRM)", "lang": "en"}, {"value": "Nicht-erneuerbare Primärenergie zur stofflichen Nutzung (PENRM)", "lang": "de"}], "type": "flow data set", "refObjectId": "1421caa0-679d-4bf4-b282-0eb850ccae27", "version": "38.00.000"}, "exchange direction": "INPUT", "meanAmount": 0.0, "other": {"anies": [{"value": "125.0", "module": "A1-A3"}, {"value": "2.19", "module": "A4"}, {"value": "0.572", "module": "A5"}, {"value": "0.0809", "module": "B2"}, {"value": "0.0816", "module": "B3"}, {"value": "134.0", "module": "B4"}, {"value": "0.0", "module": "C1"}, {"value": "0.215", "module": "C2"}, {"value": "1.27", "module": "C3"}, {"value": "0.151", "module": "C4"}, {"value": "-18.1", "module": "D"}, {"name": "referenceToUnitGroupDataSet", "value": {"shortDescription": [{"value": "MJ"}], "type": "unit group data set", "refObjectId": "93a60a57-a3c8-11da-a746-0800200c9a66", "uri": "../unitgroups/93a60a57-a3c8-11da-a746-0800200c9a66"}}]}, "flowProperties": [], "typeOfFlow": "Other flow", "classification": {"classHierarchy": "Quantities", "name": "GaBiCategories"}}, {"dataSetInternalID": 12, "referenceToFlowDataSet": {"shortDescription": [{"value": "Use of non renewable secondary fuels (NRSF)", "lang": "en"}, {"value": "Verbrauch nicht erneuerbarer Sekundärbrennstoffe (NRSF)", "lang": "de"}], "type": "flow data set", "refObjectId": "89def144-d39a-4287-b86f-efde453ddcb2", "version": "38.00.000"}, "exchange direction": "INPUT", "meanAmount": 0.0, "other": {"anies": [{"value": "0.0", "module": "A1-A3"}, {"value": "0.0", "module": "A4"}, {"value": "0.0", "module": "A5"}, {"value": "0.0", "module": "B2"}, {"value": "0.0", "module": "B3"}, {"value": "0.0", "module": "B4"}, {"value": "0.0", "module": "C1"}, {"value": "0.0", "module": "C2"}, {"value": "0.0", "module": "C3"}, {"value": "0.0", "module": "C4"}, {"value": "0.0", "module": "D"}, {"name": "referenceToUnitGroupDataSet", "value": {"shortDescription": [{"value": "MJ"}], "type": "unit group data set", "refObjectId": "93a60a57-a3c8-11da-a746-0800200c9a66", "uri": "../unitgroups/93a60a57-a3c8-11da-a746-0800200c9a66"}}]}, "flowProperties": [], "typeOfFlow": "Other flow", "classification": {"classHierarchy": "Quantities / Environmental quantities / EPD EN 15804 / LCI indicators", "name": "GaBiCategories"}}, {"dataSetInternalID": 13, "referenceToFlowDataSet": {"shortDescription": [{"value": "Radioactive waste disposed (RWD)", "lang": "en"}, {"value": "Entsorgter radioaktiver Abfall (RWD)", "lang": "de"}], "type": "flow data set", "refObjectId": "3449546e-52ad-4b39-b809-9fb77cea8ff6", "version": "38.00.000"}, "exchange direction": "OUTPUT", "meanAmount": 0.0, "other": {"anies": [{"value": "0.00402", "module": "A1-A3"}, {"value": "9.69E-6", "module": "A4"}, {"value": "4.94E-5", "module": "A5"}, {"value": "9.38E-7", "module": "B2"}, {"value": "6.01E-6", "module": "B3"}, {"value": "0.00416", "module": "B4"}, {"value": "0.0", "module": "C1"}, {"value": "6.93E-7", "module": "C2"}, {"value": "6.15E-5", "module": "C3"}, {"value": "5.6E-7", "module": "C4"}, {"value": "-0.00105", "module": "D"}, {"name": "referenceToUnitGroupDataSet", "value": {"shortDescription": [{"value": "kg"}], "type": "unit group data set", "refObjectId": "ad38d542-3fe9-439d-9b95-2f5f7752acaf", "uri": "../unitgroups/ad38d542-3fe9-439d-9b95-2f5f7752acaf"}}]}, "flowProperties": [], "typeOfFlow": "Other flow", "classification": {"classHierarchy": "Quantities / Environmental quantities / EPD EN 15804 / LCI indicators", "name": "GaBiCategories"}}, {"dataSetInternalID": 14, "referenceToFlowDataSet": {"shortDescription": [{"value": "Erneuerbare Primärenergie als Energieträger (PERE)", "lang": "en"}, {"value": "Erneuerbare Primärenergie als Energieträger (PERE)", "lang": "de"}], "type": "flow data set", "refObjectId": "20f32be5-0398-4288-9b6d-accddd195317", "version": "38.00.000"}, "exchange direction": "INPUT", "meanAmount": 0.0, "other": {"anies": [{"value": "1250.0", "module": "A1-A3"}, {"value": "0.498", "module": "A4"}, {"value": "0.882", "module": "A5"}, {"value": "0.203", "module": "B2"}, {"value": "0.487", "module": "B3"}, {"value": "1260.0", "module": "B4"}, {"value": "0.0", "module": "C1"}, {"value": "0.0366", "module": "C2"}, {"value": "3.58", "module": "C3"}, {"value": "0.043", "module": "C4"}, {"value": "-81.2", "module": "D"}, {"name": "referenceToUnitGroupDataSet", "value": {"shortDescription": [{"value": "MJ"}], "type": "unit group data set", "refObjectId": "93a60a57-a3c8-11da-a746-0800200c9a66", "uri": "../unitgroups/93a60a57-a3c8-11da-a746-0800200c9a66"}}]}, "flowProperties": [], "typeOfFlow": "Other flow", "classification": {"classHierarchy": "Quantities", "name": "GaBiCategories"}}, {"dataSetInternalID": 15, "referenceToFlowDataSet": {"shortDescription": [{"value": "Erneuerbare Primärenergie zur stofflichen Nutzung (PERM)", "lang": "en"}, {"value": "Erneuerbare Primärenergie zur stofflichen Nutzung (PERM)", "lang": "de"}], "type": "flow data set", "refObjectId": "fb3ec0de-548d-4508-aea5-00b73bf6f702", "version": "38.00.000"}, "exchange direction": "INPUT", "meanAmount": 0.0, "other": {"anies": [{"value": "0.0", "module": "A1-A3"}, {"value": "0.0", "module": "A4"}, {"value": "0.0", "module": "A5"}, {"value": "0.0", "module": "B2"}, {"value": "0.0", "module": "B3"}, {"value": "0.0", "module": "B4"}, {"value": "0.0", "module": "C1"}, {"value": "0.0", "module": "C2"}, {"value": "0.0", "module": "C3"}, {"value": "0.0", "module": "C4"}, {"value": "0.0", "module": "D"}, {"name": "referenceToUnitGroupDataSet", "value": {"shortDescription": [{"value": "MJ"}], "type": "unit group data set", "refObjectId": "93a60a57-a3c8-11da-a746-0800200c9a66", "uri": "../unitgroups/93a60a57-a3c8-11da-a746-0800200c9a66"}}]}, "flowProperties": [], "typeOfFlow": "Other flow", "classification": {"classHierarchy": "Quantities", "name": "GaBiCategories"}}, {"dataSetInternalID": 16, "referenceToFlowDataSet": {"shortDescription": [{"value": "Use of renewable secondary fuels (RSF)", "lang": "en"}, {"value": "Erneuerbare Sekundärbrennstoffe (RSF)", "lang": "de"}], "type": "flow data set", "refObjectId": "64333088-a55f-4aa2-9a31-c10b07816787", "version": "38.00.000"}, "exchange direction": "INPUT", "meanAmount": 0.0, "other": {"anies": [{"value": "3.95", "module": "A1-A3"}, {"value": "0.0104", "module": "A4"}, {"value": "0.00869", "module": "A5"}, {"value": "8.26E-4", "module": "B2"}, {"value": "0.00487", "module": "B3"}, {"value": "4.06", "module": "B4"}, {"value": "0.0", "module": "C1"}, {"value": "6.1E-4", "module": "C2"}, {"value": "0.0639", "module": "C3"}, {"value": "8.43E-4", "module": "C4"}, {"value": "-0.492", "module": "D"}, {"name": "referenceToUnitGroupDataSet", "value": {"shortDescription": [{"value": "MJ"}], "type": "unit group data set", "refObjectId": "93a60a57-a3c8-11da-a746-0800200c9a66", "uri": "../unitgroups/93a60a57-a3c8-11da-a746-0800200c9a66"}}]}, "flowProperties": [], "typeOfFlow": "Other flow", "classification": {"classHierarchy": "Quantities / Environmental quantities / EPD EN 15804 / LCI indicators", "name": "GaBiCategories"}}, {"dataSetInternalID": 17, "referenceToFlowDataSet": {"shortDescription": [{"value": "Input of secondary material (SM)", "lang": "en"}, {"value": "Einsatz von Sekundärstoffen (SM)", "lang": "de"}], "type": "flow data set", "refObjectId": "c6a1f35f-2d09-4f54-8dfb-97e502e1ce92", "version": "38.00.000"}, "exchange direction": "INPUT", "meanAmount": 0.0, "other": {"anies": [{"value": "15.8", "module": "A1-A3"}, {"value": "0.0329", "module": "A4"}, {"value": "0.0999", "module": "A5"}, {"value": "0.00312", "module": "B2"}, {"value": "0.0382", "module": "B3"}, {"value": "22.0", "module": "B4"}, {"value": "0.0", "module": "C1"}, {"value": "0.0024", "module": "C2"}, {"value": "6.02", "module": "C3"}, {"value": "0.00226", "module": "C4"}, {"value": "-4.19", "module": "D"}, {"name": "referenceToUnitGroupDataSet", "value": {"shortDescription": [{"value": "kg"}], "type": "unit group data set", "refObjectId": "ad38d542-3fe9-439d-9b95-2f5f7752acaf", "uri": "../unitgroups/ad38d542-3fe9-439d-9b95-2f5f7752acaf"}}]}, "flowProperties": [], "typeOfFlow": "Other flow", "classification": {"classHierarchy": "Quantities / Environmental quantities / EPD EN 15804 / LCI indicators", "name": "GaBiCategories"}}, {"dataSetInternalID": 18, "referenceToFlowDataSet": {"shortDescription": [{"value": "Total use of non-renewable primary energy resources (PENRT)", "lang": "en"}, {"value": "Total nicht erneuerbare Primärenergie (PENRT)", "lang": "de"}], "type": "flow data set", "refObjectId": "06159210-646b-4c8d-8583-da9b3b95a6c1", "version": "38.00.000"}, "exchange direction": "INPUT", "meanAmount": 0.0, "other": {"anies": [{"value": "2630.0", "module": "A1-A3"}, {"value": "23.8", "module": "A4"}, {"value": "23.3", "module": "A5"}, {"value": "1.18", "module": "B2"}, {"value": "2.31", "module": "B3"}, {"value": "2770.0", "module": "B4"}, {"value": "0.0", "module": "C1"}, {"value": "2.31", "module": "C2"}, {"value": "29.6", "module": "C3"}, {"value": "1.62", "module": "C4"}, {"value": "-587.0", "module": "D"}, {"name": "referenceToUnitGroupDataSet", "value": {"shortDescription": [{"value": "MJ"}], "type": "unit group data set", "refObjectId": "93a60a57-a3c8-11da-a746-0800200c9a66", "uri": "../unitgroups/93a60a57-a3c8-11da-a746-0800200c9a66"}}]}, "flowProperties": [], "typeOfFlow": "Other flow", "classification": {"classHierarchy": "Quantities / Environmental quantities / EPD EN 15804 / LCI indicators", "name": "GaBiCategories"}}, {"dataSetInternalID": 19, "referenceToFlowDataSet": {"shortDescription": [{"value": "Total use of renewable primary energy resources (PERT)", "lang": "en"}, {"value": "Gesamtverbrauch von erneuerbarer Primärenergie (PERT)", "lang": "de"}], "type": "flow data set", "refObjectId": "53f97275-fa8a-4cdd-9024-65936002acd0", "version": "38.00.000"}, "exchange direction": "INPUT", "meanAmount": 0.0, "other": {"anies": [{"value": "1250.0", "module": "A1-A3"}, {"value": "0.498", "module": "A4"}, {"value": "0.882", "module": "A5"}, {"value": "0.203", "module": "B2"}, {"value": "0.487", "module": "B3"}, {"value": "1260.0", "module": "B4"}, {"value": "0.0", "module": "C1"}, {"value": "0.0366", "module": "C2"}, {"value": "3.58", "module": "C3"}, {"value": "0.043", "module": "C4"}, {"value": "-81.2", "module": "D"}, {"name": "referenceToUnitGroupDataSet", "value": {"shortDescription": [{"value": "MJ"}], "type": "unit group data set", "refObjectId": "93a60a57-a3c8-11da-a746-0800200c9a66", "uri": "../unitgroups/93a60a57-a3c8-11da-a746-0800200c9a66"}}]}, "flowProperties": [], "typeOfFlow": "Other flow", "classification": {"classHierarchy": "Quantities / Environmental quantities / EPD EN 15804 / LCI indicators", "name": "GaBiCategories"}}]}, "LCIAResults": {"LCIAResult": [{"referenceToLCIAMethodDataSet": {"shortDescription": [{"value": "Abiotic depletion potential - non-fossil resources (ADPE)", "lang": "en"}, {"value": "Potenzial für die Verknappung abiotischer Ressourcen – nicht fossile Ressourcen (ADPE)", "lang": "de"}], "type": "LCIA method data set", "refObjectId": "b2ad6494-c78d-11e6-9d9d-cec0c932ce01", "version": "01.00.011"}, "meanAmount": 0.0, "other": {"anies": [{"value": "0.00333", "module": "A1-A3"}, {"value": "6.47E-6", "module": "A4"}, {"value": "9.92E-6", "module": "A5"}, {"value": "5.81E-7", "module": "B2"}, {"value": "2.44E-5", "module": "B3"}, {"value": "0.0034", "module": "B4"}, {"value": "0.0", "module": "C1"}, {"value": "4.4E-7", "module": "C2"}, {"value": "2.13E-5", "module": "C3"}, {"value": "1.52E-7", "module": "C4"}, {"value": "-0.00117", "module": "D"}, {"name": "referenceToUnitGroupDataSet", "value": {"shortDescription": [{"value": "kg Sb-Äqv."}], "type": "unit group data set", "refObjectId": "54ccd2d9-a32a-4fc2-923d-f2c8c93e89d4", "uri": "../unitgroups/54ccd2d9-a32a-4fc2-923d-f2c8c93e89d4"}}]}}, {"referenceToLCIAMethodDataSet": {"shortDescription": [{"value": "Abiotic depletion potential - fossil resources (ADPF)", "lang": "en"}, {"value": "Potenzial für die Verknappung abiotischer Ressourcen – fossile Brennstoffe (ADPF)", "lang": "de"}], "type": "LCIA method data set", "refObjectId": "b2ad6110-c78d-11e6-9d9d-cec0c932ce01", "version": "01.00.011"}, "meanAmount": 0.0, "other": {"anies": [{"value": "2630.0", "module": "A1-A3"}, {"value": "23.8", "module": "A4"}, {"value": "23.3", "module": "A5"}, {"value": "1.18", "module": "B2"}, {"value": "2.31", "module": "B3"}, {"value": "2770.0", "module": "B4"}, {"value": "0.0", "module": "C1"}, {"value": "2.31", "module": "C2"}, {"value": "29.6", "module": "C3"}, {"value": "1.62", "module": "C4"}, {"value": "-587.0", "module": "D"}, {"name": "referenceToUnitGroupDataSet", "value": {"shortDescription": [{"value": "MJ"}], "type": "unit group data set", "refObjectId": "93a60a57-a3c8-11da-a746-0800200c9a66", "uri": "../unitgroups/93a60a57-a3c8-11da-a746-0800200c9a66"}}]}}, {"referenceToLCIAMethodDataSet": {"shortDescription": [{"value": "Acidification potential, Accumulated Exceedance (AP)", "lang": "en"}, {"value": "Versauerungspotenzial, kumulierte Überschreitung (AP)", "lang": "de"}], "type": "LCIA method data set", "refObjectId": "b5c611c6-def3-11e6-bf01-fe55135034f3", "version": "01.03.010", "uri": "http://lca.jrc.ec.europa.eu/lcainfohub/datasets/elcd/lciamethods/f6cbd466-253f-4145-a4bb-8dae7d266e89.xml"}, "meanAmount": 0.0, "other": {"anies": [{"value": "0.708", "module": "A1-A3"}, {"value": "0.00356", "module": "A4"}, {"value": "0.00695", "module": "A5"}, {"value": "2.95E-4", "module": "B2"}, {"value": "0.00157", "module": "B3"}, {"value": "0.746", "module": "B4"}, {"value": "0.0", "module": "C1"}, {"value": "3.63E-4", "module": "C2"}, {"value": "0.0167", "module": "C3"}, {"value": "4.8E-4", "module": "C4"}, {"value": "-0.209", "module": "D"}, {"name": "referenceToUnitGroupDataSet", "value": {"shortDescription": [{"value": "mol H+ eqv."}], "type": "unit group data set", "refObjectId": "42e089ac-92bf-4bf2-8ca1-5fc40d18f2ed", "uri": "../unitgroups/42e089ac-92bf-4bf2-8ca1-5fc40d18f2ed"}}]}}, {"referenceToLCIAMethodDataSet": {"shortDescription": [{"value": "Eutrophication potential - freshwater (EP-freshwater)", "lang": "en"}, {"value": "Eutrophierungspotenzial - Süßwasser (EP-freshwater)", "lang": "de"}], "type": "LCIA method data set", "refObjectId": "b53ec18f-7377-4ad3-86eb-cc3f4f276b2b", "version": "01.00.011", "uri": "http://lca.jrc.ec.europa.eu/lcainfohub/datasets/elcd/lciamethods/a4630d5b-df2f-48ae-b3f2-5e5257606d68.xml"}, "meanAmount": 0.0, "other": {"anies": [{"value": "0.0469", "module": "A1-A3"}, {"value": "1.27E-4", "module": "A4"}, {"value": "7.6E-4", "module": "A5"}, {"value": "1.54E-5", "module": "B2"}, {"value": "1.27E-4", "module": "B3"}, {"value": "0.0491", "module": "B4"}, {"value": "0.0", "module": "C1"}, {"value": "1.08E-5", "module": "C2"}, {"value": "8.99E-4", "module": "C3"}, {"value": "6.21E-6", "module": "C4"}, {"value": "-0.0171", "module": "D"}, {"name": "referenceToUnitGroupDataSet", "value": {"shortDescription": [{"value": "kg P eqv."}], "type": "unit group data set", "refObjectId": "0429039d-a61d-4590-ba67-aa4a20a810a1", "uri": "../unitgroups/0429039d-a61d-4590-ba67-aa4a20a810a1"}}]}}, {"referenceToLCIAMethodDataSet": {"shortDescription": [{"value": "Eutrophication potential - marine (EP-marine)", "lang": "en"}, {"value": "Eutrophierungspotenzial - Salzwasser (EP-marine)", "lang": "de"}], "type": "LCIA method data set", "refObjectId": "b5c619fa-def3-11e6-bf01-fe55135034f3", "version": "02.00.011", "uri": "http://lca.jrc.ec.europa.eu/lcainfohub/datasets/elcd/lciamethods/5296e2be-060b-4e50-b033-d45f85f6ac92.xml"}, "meanAmount": 0.0, "other": {"anies": [{"value": "0.139", "module": "A1-A3"}, {"value": "8.41E-4", "module": "A4"}, {"value": "0.00189", "module": "A5"}, {"value": "8.43E-5", "module": "B2"}, {"value": "2.3E-4", "module": "B3"}, {"value": "0.164", "module": "B4"}, {"value": "0.0", "module": "C1"}, {"value": "9.53E-5", "module": "C2"}, {"value": "0.00669", "module": "C3"}, {"value": "0.0127", "module": "C4"}, {"value": "-0.0389", "module": "D"}, {"name": "referenceToUnitGroupDataSet", "value": {"shortDescription": [{"value": "kg N eqv."}], "type": "unit group data set", "refObjectId": "d05bb823-ecdf-4686-8c40-bf1d9257859f", "uri": "../unitgroups/d05bb823-ecdf-4686-8c40-bf1d9257859f"}}]}}, {"referenceToLCIAMethodDataSet": {"shortDescription": [{"value": "Eutrophication potential - terrestrial (EP-terrestrial)", "lang": "en"}, {"value": "Eutrophierungspotenzial - Land (EP-terrestrial)", "lang": "de"}], "type": "LCIA method data set", "refObjectId": "b5c614d2-def3-11e6-bf01-fe55135034f3", "version": "01.02.010", "uri": "http://lca.jrc.ec.europa.eu/lcainfohub/datasets/elcd/lciamethods/40054970-5936-477c-9bec-29fa23b1cb77.xml"}, "meanAmount": 0.0, "other": {"anies": [{"value": "1.4", "module": "A1-A3"}, {"value": "0.00908", "module": "A4"}, {"value": "0.0189", "module": "A5"}, {"value": "6.01E-4", "module": "B2"}, {"value": "0.00245", "module": "B3"}, {"value": "1.52", "module": "B4"}, {"value": "0.0", "module": "C1"}, {"value": "0.00103", "module": "C2"}, {"value": "0.0568", "module": "C3"}, {"value": "0.00209", "module": "C4"}, {"value": "-0.408", "module": "D"}, {"name": "referenceToUnitGroupDataSet", "value": {"shortDescription": [{"value": "mol N eqv."}], "type": "unit group data set", "refObjectId": "71b4d617-0ec9-4d3f-b65e-e438940c2401", "uri": "../unitgroups/71b4d617-0ec9-4d3f-b65e-e438940c2401"}}]}}, {"referenceToLCIAMethodDataSet": {"shortDescription": [{"value": "Global Warming Potential - total (GWP-total)", "lang": "en"}, {"value": "Globales Erwärmungspotenzial - total (GWP-total)", "lang": "de"}], "type": "LCIA method data set", "refObjectId": "6a37f984-a4b3-458a-a20a-64418c145fa2", "version": "04.00.017"}, "meanAmount": 0.0, "other": {"anies": [{"value": "114.0", "module": "A1-A3"}, {"value": "1.66", "module": "A4"}, {"value": "13.6", "module": "A5"}, {"value": "0.0443", "module": "B2"}, {"value": "0.188", "module": "B3"}, {"value": "164.0", "module": "B4"}, {"value": "0.0", "module": "C1"}, {"value": "0.154", "module": "C2"}, {"value": "30.0", "module": "C3"}, {"value": "0.433", "module": "C4"}, {"value": "-47.6", "module": "D"}, {"name": "referenceToUnitGroupDataSet", "value": {"shortDescription": [{"value": "kg CO2-Äqv."}], "type": "unit group data set", "refObjectId": "1ebf3012-d0db-4de2-aefd-ef30cedb0be1", "uri": "../unitgroups/1ebf3012-d0db-4de2-aefd-ef30cedb0be1"}}]}}, {"referenceToLCIAMethodDataSet": {"shortDescription": [{"value": "Global Warming Potential - fossil fuels (GWP-fossil)", "lang": "en"}, {"value": "Globales Erwärmungspotenzial - fossil (GWP-fossil)", "lang": "de"}], "type": "LCIA method data set", "refObjectId": "5f635281-343e-44fb-83df-1971b155e6b6", "version": "01.00.009"}, "meanAmount": 0.0, "other": {"anies": [{"value": "160.0", "module": "A1-A3"}, {"value": "1.66", "module": "A4"}, {"value": "2.14", "module": "A5"}, {"value": "0.0495", "module": "B2"}, {"value": "0.181", "module": "B3"}, {"value": "198.0", "module": "B4"}, {"value": "0.0", "module": "C1"}, {"value": "0.154", "module": "C2"}, {"value": "29.8", "module": "C3"}, {"value": "0.432", "module": "C4"}, {"value": "-47.3", "module": "D"}, {"name": "referenceToUnitGroupDataSet", "value": {"shortDescription": [{"value": "kg CO2-Äqv."}], "type": "unit group data set", "refObjectId": "1ebf3012-d0db-4de2-aefd-ef30cedb0be1", "uri": "../unitgroups/1ebf3012-d0db-4de2-aefd-ef30cedb0be1"}}]}}, {"referenceToLCIAMethodDataSet": {"shortDescription": [{"value": "Global Warming Potential - biogenic (GWP-biogenic)", "lang": "en"}, {"value": "Globales Erwärmungspotenzial - biogen (GWP-biogenic)", "lang": "de"}], "type": "LCIA method data set", "refObjectId": "2356e1ab-0185-4db5-86e5-16de51c7485c", "version": "01.00.006"}, "meanAmount": 0.0, "other": {"anies": [{"value": "-45.8", "module": "A1-A3"}, {"value": "0.00102", "module": "A4"}, {"value": "11.5", "module": "A5"}, {"value": "-0.00784", "module": "B2"}, {"value": "0.00642", "module": "B3"}, {"value": "-34.2", "module": "B4"}, {"value": "0.0", "module": "C1"}, {"value": "8.22E-5", "module": "C2"}, {"value": "0.208", "module": "C3"}, {"value": "6.43E-4", "module": "C4"}, {"value": "-0.294", "module": "D"}, {"name": "referenceToUnitGroupDataSet", "value": {"shortDescription": [{"value": "kg CO2-Äqv."}], "type": "unit group data set", "refObjectId": "1ebf3012-d0db-4de2-aefd-ef30cedb0be1", "uri": "../unitgroups/1ebf3012-d0db-4de2-aefd-ef30cedb0be1"}}]}}, {"referenceToLCIAMethodDataSet": {"shortDescription": [{"value": "Global Warming Potential - land use and land use change (GWP-luluc)", "lang": "en"}, {"value": "Globales Erwärmungspotenzial - luluc (GWP-luluc)", "lang": "de"}], "type": "LCIA method data set", "refObjectId": "4331bbdb-978a-490d-8707-eeb047f01a55", "version": "01.00.006"}, "meanAmount": 0.0, "other": {"anies": [{"value": "0.162", "module": "A1-A3"}, {"value": "6.19E-4", "module": "A4"}, {"value": "7.05E-4", "module": "A5"}, {"value": "0.00256", "module": "B2"}, {"value": "2.35E-4", "module": "B3"}, {"value": "0.169", "module": "B4"}, {"value": "0.0", "module": "C1"}, {"value": "5.45E-5", "module": "C2"}, {"value": "0.00221", "module": "C3"}, {"value": "2.01E-5", "module": "C4"}, {"value": "-0.0255", "module": "D"}, {"name": "referenceToUnitGroupDataSet", "value": {"shortDescription": [{"value": "kg CO2-Äqv."}], "type": "unit group data set", "refObjectId": "1ebf3012-d0db-4de2-aefd-ef30cedb0be1", "uri": "../unitgroups/1ebf3012-d0db-4de2-aefd-ef30cedb0be1"}}]}}, {"referenceToLCIAMethodDataSet": {"shortDescription": [{"value": "Depletion potential of the stratospheric ozone layer (ODP)", "lang": "en"}, {"value": "Abbaupotenzial der stratosphärischen Ozonschicht (ODP)", "lang": "de"}], "type": "LCIA method data set", "refObjectId": "b5c629d6-def3-11e6-bf01-fe55135034f3", "version": "02.00.013", "uri": "http://lca.jrc.ec.europa.eu/lcainfohub/datasets/elcd/lciamethods/8b723200-3d8f-4eec-9e10-444edb029476.xml"}, "meanAmount": 0.0, "other": {"anies": [{"value": "2.78E-6", "module": "A1-A3"}, {"value": "3.34E-8", "module": "A4"}, {"value": "1.63E-8", "module": "A5"}, {"value": "1.71E-9", "module": "B2"}, {"value": "1.93E-9", "module": "B3"}, {"value": "2.95E-6", "module": "B4"}, {"value": "0.0", "module": "C1"}, {"value": "3.2E-9", "module": "C2"}, {"value": "3.62E-8", "module": "C3"}, {"value": "2.2E-9", "module": "C4"}, {"value": "-5.08E-7", "module": "D"}, {"name": "referenceToUnitGroupDataSet", "value": {"shortDescription": [{"value": "kg CFC 11-Äquiv."}], "type": "unit group data set", "refObjectId": "d9e957c9-7309-4474-bf3a-7777df6c4e5b", "uri": "../unitgroups/d9e957c9-7309-4474-bf3a-7777df6c4e5b"}}]}}, {"referenceToLCIAMethodDataSet": {"shortDescription": [{"value": "Photochemical Ozone Creation Potential (POCP)", "lang": "en"}, {"value": "Bildungspotenzial für troposphärisches Ozon (POCP)", "lang": "de"}], "type": "LCIA method data set", "refObjectId": "b5c610fe-def3-11e6-bf01-fe55135034f3", "version": "02.00.015", "uri": "http://lca.jrc.ec.europa.eu/lcainfohub/datasets/elcd/lciamethods/ec7836be-83eb-41da-bcda-1a6a3fe2d149.xml"}, "meanAmount": 0.0, "other": {"anies": [{"value": "0.584", "module": "A1-A3"}, {"value": "0.00585", "module": "A4"}, {"value": "0.00539", "module": "A5"}, {"value": "4.61E-4", "module": "B2"}, {"value": "7.47E-4", "module": "B3"}, {"value": "0.628", "module": "B4"}, {"value": "0.0", "module": "C1"}, {"value": "6.3E-4", "module": "C2"}, {"value": "0.0158", "module": "C3"}, {"value": "8.69E-4", "module": "C4"}, {"value": "-0.131", "module": "D"}, {"name": "referenceToUnitGroupDataSet", "value": {"shortDescription": [{"value": "kg NMVOC eqv."}], "type": "unit group data set", "refObjectId": "d27c25f8-fbc1-44c6-b47b-4adbae4199c6", "uri": "../unitgroups/d27c25f8-fbc1-44c6-b47b-4adbae4199c6"}}]}}, {"referenceToLCIAMethodDataSet": {"shortDescription": [{"value": "Water (user) deprivation potential (WDP)", "lang": "en"}, {"value": "Wasser-Entzugspotenzial (Benutzer) (WDP)", "lang": "de"}], "type": "LCIA method data set", "refObjectId": "b2ad66ce-c78d-11e6-9d9d-cec0c932ce01", "version": "03.00.015"}, "meanAmount": 0.0, "other": {"anies": [{"value": "53.5", "module": "A1-A3"}, {"value": "0.129", "module": "A4"}, {"value": "0.467", "module": "A5"}, {"value": "0.0468", "module": "B2"}, {"value": "0.0847", "module": "B3"}, {"value": "63.1", "module": "B4"}, {"value": "0.0", "module": "C1"}, {"value": "0.0116", "module": "C2"}, {"value": "8.58", "module": "C3"}, {"value": "0.0102", "module": "C4"}, {"value": "-9.73", "module": "D"}, {"name": "referenceToUnitGroupDataSet", "value": {"shortDescription": [{"value": "m3 world eqv."}], "type": "unit group data set", "refObjectId": "6ae2df01-888e-46c8-b17d-49fa3869b476", "uri": "../unitgroups/6ae2df01-888e-46c8-b17d-49fa3869b476"}}]}}, {"referenceToLCIAMethodDataSet": {"shortDescription": [{"value": "Potential incidence of disease due to PM emissions (PM)", "lang": "en"}, {"value": "Potenzielles Auftreten von Krankheiten aufgrund von Feinstaubemissionen (PM)", "lang": "de"}], "type": "LCIA method data set", "refObjectId": "b5c602c6-def3-11e6-bf01-fe55135034f3", "version": "02.00.012", "uri": "http://lca.jrc.ec.europa.eu/lcainfohub/datasets/elcd/lciamethods/72ce3013-f678-4c6a-935b-f4752ff8901b.xml"}, "meanAmount": 0.0, "other": {"anies": [{"value": "9.52E-6", "module": "A1-A3"}, {"value": "1.14E-7", "module": "A4"}, {"value": "4.96E-8", "module": "A5"}, {"value": "3.12E-9", "module": "B2"}, {"value": "1.32E-8", "module": "B3"}, {"value": "1.02E-5", "module": "B4"}, {"value": "0.0", "module": "C1"}, {"value": "1.5E-8", "module": "C2"}, {"value": "1.28E-7", "module": "C3"}, {"value": "1.11E-8", "module": "C4"}, {"value": "-2.45E-6", "module": "D"}, {"name": "referenceToUnitGroupDataSet", "value": {"shortDescription": [{"value": "disease incidence"}], "type": "unit group data set", "refObjectId": "3883559b-648f-4afc-8ba2-0bd24f3affa3", "uri": "../unitgroups/3883559b-648f-4afc-8ba2-0bd24f3affa3"}}]}}, {"referenceToLCIAMethodDataSet": {"shortDescription": [{"value": "Potential Human exposure efficiency relative to U235 (IRP)", "lang": "en"}, {"value": "Potenzielle Wirkung durch Exposition des Menschen mit U235 (IRP)", "lang": "de"}], "type": "LCIA method data set", "refObjectId": "b5c632be-def3-11e6-bf01-fe55135034f3", "version": "01.00.012", "uri": "http://lca.jrc.ec.europa.eu/lcainfohub/datasets/elcd/lciamethods/a6f4cbc8-5388-44d6-9a67-53d05684f93e.xml"}, "meanAmount": 0.0, "other": {"anies": [{"value": "15.4", "module": "A1-A3"}, {"value": "0.0388", "module": "A4"}, {"value": "0.174", "module": "A5"}, {"value": "0.0037", "module": "B2"}, {"value": "0.0236", "module": "B3"}, {"value": "15.9", "module": "B4"}, {"value": "0.0", "module": "C1"}, {"value": "0.0028", "module": "C2"}, {"value": "0.247", "module": "C3"}, {"value": "0.00239", "module": "C4"}, {"value": "-3.86", "module": "D"}, {"name": "referenceToUnitGroupDataSet", "value": {"shortDescription": [{"value": "kBq U235 eqv."}], "type": "unit group data set", "refObjectId": "456b05bf-1415-44a9-9993-02452f554c09", "uri": "../unitgroups/456b05bf-1415-44a9-9993-02452f554c09"}}]}}, {"referenceToLCIAMethodDataSet": {"shortDescription": [{"value": "Potential Comparative Toxic Unit for ecosystems (ETP-fw)", "lang": "en"}, {"value": "Potenzielle Toxizitätsvergleichseinheit für Ökosysteme (ETP-fw)", "lang": "de"}], "type": "LCIA method data set", "refObjectId": "ee1082d1-b0f7-43ca-a1f0-21e2a4a74511", "version": "01.00.003", "uri": "http://lca.jrc.ec.europa.eu/lcainfohub/datasets/elcd/lciamethods/ee1082d1-b0f7-43ca-a1f0-21e2a4a74511.xml"}, "meanAmount": 0.0, "other": {"anies": [{"value": "1860.0", "module": "A1-A3"}, {"value": "7.01", "module": "A4"}, {"value": "6.32", "module": "A5"}, {"value": "0.574", "module": "B2"}, {"value": "6.01", "module": "B3"}, {"value": "2270.0", "module": "B4"}, {"value": "0.0", "module": "C1"}, {"value": "0.546", "module": "C2"}, {"value": "370.0", "module": "C3"}, {"value": "10.8", "module": "C4"}, {"value": "-410.0", "module": "D"}, {"name": "referenceToUnitGroupDataSet", "value": {"shortDescription": [{"value": "CTUe"}], "type": "unit group data set", "refObjectId": "aa959ded-f1eb-4efb-9c5c-2d60be36b3e6", "uri": "../unitgroups/aa959ded-f1eb-4efb-9c5c-2d60be36b3e6"}}]}}, {"referenceToLCIAMethodDataSet": {"shortDescription": [{"value": "Potential Comparative Toxic Unit for humans - cancer effects (HTP-c)", "lang": "en"}, {"value": "Potenzielle Toxizitätsvergleichseinheit für den Menschen - kanzerogene Wirkung (HTP-c)", "lang": "de"}], "type": "LCIA method data set", "refObjectId": "2299222a-bbd8-474f-9d4f-4dd1f18aea7c", "version": "01.00.004", "uri": "http://lca.jrc.ec.europa.eu/lcainfohub/datasets/elcd/lciamethods/2299222a-bbd8-474f-9d4f-4dd1f18aea7c.xml"}, "meanAmount": 0.0, "other": {"anies": [{"value": "1.67E-6", "module": "A1-A3"}, {"value": "1.2E-8", "module": "A4"}, {"value": "4.73E-9", "module": "A5"}, {"value": "2.62E-10", "module": "B2"}, {"value": "3.81E-9", "module": "B3"}, {"value": "1.73E-6", "module": "B4"}, {"value": "0.0", "module": "C1"}, {"value": "9.84E-10", "module": "C2"}, {"value": "1.23E-8", "module": "C3"}, {"value": "4.01E-10", "module": "C4"}, {"value": "-7.63E-7", "module": "D"}, {"name": "referenceToUnitGroupDataSet", "value": {"shortDescription": [{"value": "CTUh"}], "type": "unit group data set", "refObjectId": "d4c9523e-2d7e-49fd-8469-998f547d3a70", "uri": "../unitgroups/d4c9523e-2d7e-49fd-8469-998f547d3a70"}}]}}, {"referenceToLCIAMethodDataSet": {"shortDescription": [{"value": "Potential Comparative Toxic Unit for humans - non-cancer effects (HTP-nc)", "lang": "en"}, {"value": "Potenzielle Toxizitätsvergleichseinheit für den Menschen - nicht kanzerogene Wirkung (HTP-nc)", "lang": "de"}], "type": "LCIA method data set", "refObjectId": "3af763a5-b7a1-48c9-9cee-1f223481fcef", "version": "01.00.003", "uri": "http://lca.jrc.ec.europa.eu/lcainfohub/datasets/elcd/lciamethods/3af763a5-b7a1-48c9-9cee-1f223481fcef.xml"}, "meanAmount": 0.0, "other": {"anies": [{"value": "2.54E-6", "module": "A1-A3"}, {"value": "1.51E-8", "module": "A4"}, {"value": "4.19E-8", "module": "A5"}, {"value": "5.95E-10", "module": "B2"}, {"value": "1.19E-8", "module": "B3"}, {"value": "2.76E-6", "module": "B4"}, {"value": "0.0", "module": "C1"}, {"value": "1.52E-9", "module": "C2"}, {"value": "1.14E-7", "module": "C3"}, {"value": "2.27E-9", "module": "C4"}, {"value": "-9.52E-7", "module": "D"}, {"name": "referenceToUnitGroupDataSet", "value": {"shortDescription": [{"value": "CTUh"}], "type": "unit group data set", "refObjectId": "d4c9523e-2d7e-49fd-8469-998f547d3a70", "uri": "../unitgroups/d4c9523e-2d7e-49fd-8469-998f547d3a70"}}]}}, {"referenceToLCIAMethodDataSet": {"shortDescription": [{"value": "Potential Soil quality index (SQP)", "lang": "en"}, {"value": "Potenzieller Bodenqualitätsindex (SQP)", "lang": "de"}], "type": "LCIA method data set", "refObjectId": "b2ad6890-c78d-11e6-9d9d-cec0c932ce01", "version": "01.00.011"}, "meanAmount": 0.0, "other": {"anies": [{"value": "6040.0", "module": "A1-A3"}, {"value": "15.1", "module": "A4"}, {"value": "4.22", "module": "A5"}, {"value": "0.593", "module": "B2"}, {"value": "1.22", "module": "B3"}, {"value": "6130.0", "module": "B4"}, {"value": "0.0", "module": "C1"}, {"value": "2.32", "module": "C2"}, {"value": "15.1", "module": "C3"}, {"value": "3.76", "module": "C4"}, {"value": "-173.0", "module": "D"}, {"name": "referenceToUnitGroupDataSet", "value": {"shortDescription": [{"value": "dimensionless"}], "type": "unit group data set", "refObjectId": "f130951c-e67f-4f7f-8dd4-665de3974e18", "uri": "../unitgroups/f130951c-e67f-4f7f-8dd4-665de3974e18"}}]}}]}, "otherAttributes": {"{http://www.okworx.com/ILCD/Extensions/2018/Profile}profile": "EN_15804_A2", "{http://www.indata.network/EPD/2019}epd-version": "1.2"}, "version": "1.1"}