{"processInformation": {"dataSetInformation": {"UUID": "b770703d-b5f8-48d9-92d1-6cf67f36e1e8", "name": {"baseName": [{"value": "Welded and zinc coated steel structures (Heidelberg Materials SBC Latvia SIA)", "lang": "en"}, {"value": "Geschweißte und verzinkte Stahlkonstruktionen (Heidelberg Materials SBC Latvia SIA)", "lang": "de"}]}, "synonyms": [{"value": "Welded and zinc coated steel structures (Heidelberg Materials SBC Latvia SIA)", "lang": "en"}], "classificationInformation": {"classification": [{"class": [{"value": "Metalle", "level": 0, "classId": "4"}, {"value": "Stahl und Eisen", "level": 1, "classId": "4.1"}, {"value": "Stahlprofile", "level": 2, "classId": "4.1.03"}], "name": "OEKOBAU.DAT"}]}, "generalComment": [{"value": "The EPD (type: Cradle to gate with options, modules C1-C4 and module D (A1-A4, C, D)) is based on LCA of the custom made welded and zinc coated steel structures, manufactured in Olaine, Latvia. The calculation is based on 1 metric ton of welded and galvanized steel structure with a share of 93,7% steel materials. Kiwa-Ecobility Experts shall not be liable with respect to manufacturer information, life cycle assessment data and evidence.", "lang": "en"}], "other": {"anies": [{"scenario": [{"description": [{"value": "All installed raw materials of the product were analysed, and the masses were determined following the allocation and cut-off requirements. Production-specific energy consumption was measured and provided by Heidelberg Materials SBC Latvia SIA. Since the production process is quite similar for all of steel products produced at the manufacturing site, the energy consumption, ancillary materials, and production waste were appropriated according to the annual use of steel materials and then declared per 1 metric ton of the products. The total annual production data is recorded to a high standard of accuracy and precision. The production waste is collected separately. As the product is marketed internationally, no country-specific waste scenario can be considered. Therefore, the waste scenarios of NMD (2022) were adopted. Module A4: This stage includes transport from the production stockyard to the construction site where the prefabricated product shall be installed. Transportation is calculated based on data from the manufacturer and scenarios with parameters described in the following tables. Module A5: not declared. Modules B1 to B7: not declared. In normal use scenario, it is assumed that no maintenance (B2), repair (B3), replacement (B4) and refurbishment (B5) are needed. C1: This module concerns the removal of a steel structure. The demolition process (C1) consumes energy in the form of diesel fuel used by building machines (e.g. lifting cranes, mobile rough terrain crane, forklift). According to Erlandsson, M. and Pettersson D. (2015) energy consumption of a demolition process is on average 12 kWh/t. At the End-of-life, C2 - C4 and D, it is assumed that steel material is separated after deconstruction. A waste scenario according to the Dutch National Environmental Database (NMD) is applied: Galvinised steel (i.a. profiles, sheets), where 95% of the end-of-life product is sent to recycling (C3) and 5% is landfilled (C4). All end-of-life products are assumed to be sent to the closest facilities (C2).", "lang": "en"}], "name": "Standard Scenario", "default": true}, {"name": "Norway Scenario", "default": false}, {"name": "Sweden Scenario", "default": false}]}, "<ns11:modules xmlns:ns11=\"http://openlca.org/epd_ilcd\" xmlns=\"http://lca.jrc.it/ILCD/Process\" xmlns:c=\"http://lca.jrc.it/ILCD/Contact\" xmlns:common=\"http://lca.jrc.it/ILCD/Common\" xmlns:epd=\"http://www.iai.kit.edu/EPD/2013\" xmlns:epd2=\"http://www.indata.network/EPD/2019\" xmlns:f=\"http://lca.jrc.it/ILCD/Flow\" xmlns:fp=\"http://lca.jrc.it/ILCD/FlowProperty\" xmlns:m=\"http://lca.jrc.it/ILCD/LCIAMethod\" xmlns:s=\"http://lca.jrc.it/ILCD/Source\" xmlns:u=\"http://lca.jrc.it/ILCD/UnitGroup\" name=\"A1\" scenario=\"Standard Scenario\"/>", "<ns11:modules xmlns:ns11=\"http://openlca.org/epd_ilcd\" xmlns=\"http://lca.jrc.it/ILCD/Process\" xmlns:c=\"http://lca.jrc.it/ILCD/Contact\" xmlns:common=\"http://lca.jrc.it/ILCD/Common\" xmlns:epd=\"http://www.iai.kit.edu/EPD/2013\" xmlns:epd2=\"http://www.indata.network/EPD/2019\" xmlns:f=\"http://lca.jrc.it/ILCD/Flow\" xmlns:fp=\"http://lca.jrc.it/ILCD/FlowProperty\" xmlns:m=\"http://lca.jrc.it/ILCD/LCIAMethod\" xmlns:s=\"http://lca.jrc.it/ILCD/Source\" xmlns:u=\"http://lca.jrc.it/ILCD/UnitGroup\" name=\"A2\" scenario=\"Standard Scenario\"/>", "<ns11:modules xmlns:ns11=\"http://openlca.org/epd_ilcd\" xmlns=\"http://lca.jrc.it/ILCD/Process\" xmlns:c=\"http://lca.jrc.it/ILCD/Contact\" xmlns:common=\"http://lca.jrc.it/ILCD/Common\" xmlns:epd=\"http://www.iai.kit.edu/EPD/2013\" xmlns:epd2=\"http://www.indata.network/EPD/2019\" xmlns:f=\"http://lca.jrc.it/ILCD/Flow\" xmlns:fp=\"http://lca.jrc.it/ILCD/FlowProperty\" xmlns:m=\"http://lca.jrc.it/ILCD/LCIAMethod\" xmlns:s=\"http://lca.jrc.it/ILCD/Source\" xmlns:u=\"http://lca.jrc.it/ILCD/UnitGroup\" name=\"A3\" scenario=\"Standard Scenario\"/>", "<ns11:modules xmlns:ns11=\"http://openlca.org/epd_ilcd\" xmlns=\"http://lca.jrc.it/ILCD/Process\" xmlns:c=\"http://lca.jrc.it/ILCD/Contact\" xmlns:common=\"http://lca.jrc.it/ILCD/Common\" xmlns:epd=\"http://www.iai.kit.edu/EPD/2013\" xmlns:epd2=\"http://www.indata.network/EPD/2019\" xmlns:f=\"http://lca.jrc.it/ILCD/Flow\" xmlns:fp=\"http://lca.jrc.it/ILCD/FlowProperty\" xmlns:m=\"http://lca.jrc.it/ILCD/LCIAMethod\" xmlns:s=\"http://lca.jrc.it/ILCD/Source\" xmlns:u=\"http://lca.jrc.it/ILCD/UnitGroup\" name=\"A4\" scenario=\"Norway Scenario\"/>", "<ns11:modules xmlns:ns11=\"http://openlca.org/epd_ilcd\" xmlns=\"http://lca.jrc.it/ILCD/Process\" xmlns:c=\"http://lca.jrc.it/ILCD/Contact\" xmlns:common=\"http://lca.jrc.it/ILCD/Common\" xmlns:epd=\"http://www.iai.kit.edu/EPD/2013\" xmlns:epd2=\"http://www.indata.network/EPD/2019\" xmlns:f=\"http://lca.jrc.it/ILCD/Flow\" xmlns:fp=\"http://lca.jrc.it/ILCD/FlowProperty\" xmlns:m=\"http://lca.jrc.it/ILCD/LCIAMethod\" xmlns:s=\"http://lca.jrc.it/ILCD/Source\" xmlns:u=\"http://lca.jrc.it/ILCD/UnitGroup\" name=\"A4\" scenario=\"Sweden Scenario\"/>", "<ns11:modules xmlns:ns11=\"http://openlca.org/epd_ilcd\" xmlns=\"http://lca.jrc.it/ILCD/Process\" xmlns:c=\"http://lca.jrc.it/ILCD/Contact\" xmlns:common=\"http://lca.jrc.it/ILCD/Common\" xmlns:epd=\"http://www.iai.kit.edu/EPD/2013\" xmlns:epd2=\"http://www.indata.network/EPD/2019\" xmlns:f=\"http://lca.jrc.it/ILCD/Flow\" xmlns:fp=\"http://lca.jrc.it/ILCD/FlowProperty\" xmlns:m=\"http://lca.jrc.it/ILCD/LCIAMethod\" xmlns:s=\"http://lca.jrc.it/ILCD/Source\" xmlns:u=\"http://lca.jrc.it/ILCD/UnitGroup\" name=\"C1\" scenario=\"Standard Scenario\"/>", "<ns11:modules xmlns:ns11=\"http://openlca.org/epd_ilcd\" xmlns=\"http://lca.jrc.it/ILCD/Process\" xmlns:c=\"http://lca.jrc.it/ILCD/Contact\" xmlns:common=\"http://lca.jrc.it/ILCD/Common\" xmlns:epd=\"http://www.iai.kit.edu/EPD/2013\" xmlns:epd2=\"http://www.indata.network/EPD/2019\" xmlns:f=\"http://lca.jrc.it/ILCD/Flow\" xmlns:fp=\"http://lca.jrc.it/ILCD/FlowProperty\" xmlns:m=\"http://lca.jrc.it/ILCD/LCIAMethod\" xmlns:s=\"http://lca.jrc.it/ILCD/Source\" xmlns:u=\"http://lca.jrc.it/ILCD/UnitGroup\" name=\"C2\" scenario=\"Standard Scenario\"/>", "<ns11:modules xmlns:ns11=\"http://openlca.org/epd_ilcd\" xmlns=\"http://lca.jrc.it/ILCD/Process\" xmlns:c=\"http://lca.jrc.it/ILCD/Contact\" xmlns:common=\"http://lca.jrc.it/ILCD/Common\" xmlns:epd=\"http://www.iai.kit.edu/EPD/2013\" xmlns:epd2=\"http://www.indata.network/EPD/2019\" xmlns:f=\"http://lca.jrc.it/ILCD/Flow\" xmlns:fp=\"http://lca.jrc.it/ILCD/FlowProperty\" xmlns:m=\"http://lca.jrc.it/ILCD/LCIAMethod\" xmlns:s=\"http://lca.jrc.it/ILCD/Source\" xmlns:u=\"http://lca.jrc.it/ILCD/UnitGroup\" name=\"C3\" scenario=\"Standard Scenario\"/>", "<ns11:modules xmlns:ns11=\"http://openlca.org/epd_ilcd\" xmlns=\"http://lca.jrc.it/ILCD/Process\" xmlns:c=\"http://lca.jrc.it/ILCD/Contact\" xmlns:common=\"http://lca.jrc.it/ILCD/Common\" xmlns:epd=\"http://www.iai.kit.edu/EPD/2013\" xmlns:epd2=\"http://www.indata.network/EPD/2019\" xmlns:f=\"http://lca.jrc.it/ILCD/Flow\" xmlns:fp=\"http://lca.jrc.it/ILCD/FlowProperty\" xmlns:m=\"http://lca.jrc.it/ILCD/LCIAMethod\" xmlns:s=\"http://lca.jrc.it/ILCD/Source\" xmlns:u=\"http://lca.jrc.it/ILCD/UnitGroup\" name=\"C4\" scenario=\"Standard Scenario\"/>", "<ns11:modules xmlns:ns11=\"http://openlca.org/epd_ilcd\" xmlns=\"http://lca.jrc.it/ILCD/Process\" xmlns:c=\"http://lca.jrc.it/ILCD/Contact\" xmlns:common=\"http://lca.jrc.it/ILCD/Common\" xmlns:epd=\"http://www.iai.kit.edu/EPD/2013\" xmlns:epd2=\"http://www.indata.network/EPD/2019\" xmlns:f=\"http://lca.jrc.it/ILCD/Flow\" xmlns:fp=\"http://lca.jrc.it/ILCD/FlowProperty\" xmlns:m=\"http://lca.jrc.it/ILCD/LCIAMethod\" xmlns:s=\"http://lca.jrc.it/ILCD/Source\" xmlns:u=\"http://lca.jrc.it/ILCD/UnitGroup\" name=\"D\" scenario=\"Standard Scenario\"/>"]}}, "quantitativeReference": {"referenceToReferenceFlow": [1], "type": "Reference flow(s)"}, "time": {"referenceYear": 2022, "dataSetValidUntil": 2029, "timeRepresentativenessDescription": [{"value": "The reference year for collecting data is 2022 (01.2022 – 12.2022).", "lang": "en"}], "other": {"anies": [{"name": "publicationDateOfEPD", "value": 1704758400000}]}}, "geography": {"locationOfOperationSupplyOrProduction": {"descriptionOfRestrictions": [{"value": "The geographical reference area is Europe or Global and can be seen in the System description boundary table.", "lang": "en"}], "location": "RER"}}, "technology": {"technologyDescriptionAndIncludedProcesses": [{"value": "Welded and zinc coated steel structures are customized construction components for many applications in the construction industry. The zinc layer is formed by immersing the steel structures into melted liquid zinc. The steel structures are manufactured according to EN 1090-2, up to EXC 4, and are CE- marked. UN CPC code: 421 Structural metal products and parts thereof. The steel structures of industrial and civil objects from SIA Heidelberg Materials SBC Latvia are made according to drawings. The manufacturing route contains the following processes: - Extraction and delivery of raw materials; - Cutting (plasma cutting, sawing, drilling etc.); - Assembling; - Welding; - Galvanizing (outsourcing); - Storage; - Transportation (delivery of finished products).", "lang": "en"}], "technologicalApplicability": [{"value": "Hot-dipped galvanized steel structures are especially appreciated in objects that are located in an aggressive, corrosion-enhancing environment. Zinc coated steel structures can be used in various areas of civil and industrial construction, for example, construction of bridges, telecommunication towers, engineering, industrial and public buildings, as well as in the agriculture and energy industry.", "lang": "en"}], "referenceToTechnologyFlowDiagrammOrPicture": [{"shortDescription": [{"value": "Flow Chart for Welded and zinc coated steel structures (Heidelberg Materials SBC Latvia SIA)", "lang": "en"}], "type": "source data set", "refObjectId": "a2f2b4d2-b4e3-4624-9159-60d498ad9bd5", "version": "00.00.001"}]}}, "modellingAndValidation": {"LCIMethodAndAllocation": {"typeOfDataSet": "EPD", "other": {"anies": [{"name": "subType", "value": "average dataset"}]}}, "dataSourcesTreatmentAndRepresentativeness": {"referenceToDataSource": [{"shortDescription": [{"value": "ecoinvent database (general)", "lang": "en"}], "type": "source data set", "refObjectId": "b497a91f-e14b-4b69-8f28-f50eb1576766", "version": "00.03.002"}, {"shortDescription": [{"value": "ecoinvent 3.6 database", "lang": "en"}], "type": "source data set", "refObjectId": "766b9973-5ee8-48a2-8098-72c8e20b369f", "version": "00.00.001"}], "useAdviceForDataSet": [{"value": "Hot-dipped galvanized steel structures are especially appreciated in objects that are located in an aggressive, corrosion-enhancing environment. Zinc coated steel structures can be used in various areas of civil and industrial construction, for example, construction of bridges, telecommunication towers, engineering, industrial and public buildings, as well as in the agriculture and energy industry.", "lang": "en"}], "other": {"anies": [{"name": "referenceToOriginalEPD", "value": {"shortDescription": {"value": "EPD for Welded and zinc coated steel structures (Heidelberg Materials SBC Latvia SIA)", "defaultValue": "EPD for Welded and zinc coated steel structures (Heidelberg Materials SBC Latvia SIA)", "lstrings": [{"lang": "en", "value": "EPD for Welded and zinc coated steel structures (Heidelberg Materials SBC Latvia SIA)"}]}, "version": {"version": 2, "majorVersion": 0, "minorVersion": 0, "subMinorVersion": 2, "zero": false, "versionString": "00.00.002"}, "type": "source data set", "uuid": {"uuid": "74be3a52-f035-407b-82c7-fc49edeac692"}, "refObjectId": "74be3a52-f035-407b-82c7-fc49edeac692", "versionAsString": "00.00.002", "resourceURLs": ["https://oekobaudat.de/OEKOBAU.DAT/resource/sources/74be3a52-f035-407b-82c7-fc49edeac692/EPD-Kiwa-EE-000369-EN.pdf?version=00.00.002"]}}]}}, "validation": {"review": [{"reviewDetails": [{"value": "Independent verification of the declaration and data according to ISO 14025:2010.", "lang": "en"}], "referenceToNameOfReviewerAndInstitution": [{"shortDescription": [{"value": "Elisabet Amat Guasch (External verifier)", "lang": "en"}], "type": "contact data set", "refObjectId": "50fe5785-3ff2-46e5-935a-dab7a249bab3", "version": "00.00.001"}], "type": "Independent external review"}]}, "complianceDeclarations": {"compliance": [{"referenceToComplianceSystem": {"shortDescription": [{"value": "ISO 14025", "lang": "en"}], "type": "source data set", "refObjectId": "4f2eb655-6e44-4874-a95a-e28f5442cd4d", "version": "00.00.001"}}, {"referenceToComplianceSystem": {"shortDescription": [{"value": "EN 15804+A2 (EF 3.0)", "lang": "de"}, {"value": "EN 15804+A2 (EF 3.0)", "lang": "en"}], "type": "source data set", "refObjectId": "c0016b33-8cf7-415c-ac6e-deba0d21440d", "version": "00.02.000"}}]}}, "administrativeInformation": {"commissionerAndGoal": {"referenceToCommissioner": [{"shortDescription": [{"value": "Heidelberg Materials SBC Latvia SIA", "lang": "en"}], "type": "contact data set", "refObjectId": "635b13ba-f8f1-45ef-af8a-ea693dd12991", "version": "00.00.001"}], "intendedApplications": [{"value": "Hot-dipped galvanized steel structures are especially appreciated in objects that are located in an aggressive, corrosion-enhancing environment. Zinc coated steel structures can be used in various areas of civil and industrial construction, for example, construction of bridges, telecommunication towers, engineering, industrial and public buildings, as well as in the agriculture and energy industry.", "lang": "en"}]}, "dataGenerator": {"referenceToPersonOrEntityGeneratingTheDataSet": [{"shortDescription": [{"value": "Kiwa GmbH (Berlin)", "lang": "en"}], "type": "contact data set", "refObjectId": "3ea4a87a-3f88-4633-b7e7-1bbdd272be43", "version": "00.00.002"}]}, "dataEntryBy": {"timeStamp": 1752581627895, "referenceToDataSetFormat": [{"shortDescription": [{"value": "EPD Data Format Extensions v1.2", "lang": "en"}, {"value": "EPD-Datenformaterweiterungen v1.2", "lang": "de"}], "type": "source data set", "refObjectId": "a29449fd-aa2f-4de8-b5d7-4b06b43c6fde", "version": "00.01.000"}, {"shortDescription": [{"value": "ILCD format", "lang": "en"}], "type": "source data set", "refObjectId": "a97a0155-0234-4b87-b4ce-a45da52f2a40", "version": "01.00.000", "uri": "http://lca.jrc.ec.europa.eu/lcainfohub/sample_data/ilcd/sources/ILCD_Format_a97a0155-0234-4b87-b4ce-a45da52f2a40_01.00.000.xml"}], "referenceToPersonOrEntityEnteringTheData": {"shortDescription": [{"value": "Kiwa GmbH (Berlin)", "lang": "en"}], "type": "contact data set", "refObjectId": "3ea4a87a-3f88-4633-b7e7-1bbdd272be43", "version": "00.00.002"}}, "publicationAndOwnership": {"dataSetVersion": "00.00.012", "referenceToRegistrationAuthority": {"shortDescription": [{"value": "Kiwa-Ecobility Experts, Kiwa GmbH (Berlin)", "lang": "en"}], "type": "contact data set", "refObjectId": "eb52a9a8-9d0f-40ce-a5c9-7b78f5615e5a", "version": "00.00.002"}, "registrationNumber": "EPD-Kiwa-EE-000369-EN", "referenceToOwnershipOfDataSet": {"shortDescription": [{"value": "Heidelberg Materials SBC Latvia SIA", "lang": "en"}], "type": "contact data set", "refObjectId": "635b13ba-f8f1-45ef-af8a-ea693dd12991", "version": "00.00.001"}, "copyright": true, "licenseType": "Free of charge for all users and uses", "accessRestrictions": [{"value": "None", "lang": "en"}], "other": {"anies": [{"name": "referenceToPublisher", "value": {"shortDescription": [{"value": "Kiwa-Ecobility Experts, Kiwa GmbH (Berlin)", "lang": "en"}], "type": "contact data set", "refObjectId": "eb52a9a8-9d0f-40ce-a5c9-7b78f5615e5a", "version": "00.00.002"}}]}}}, "exchanges": {"exchange": [{"dataSetInternalID": 1, "referenceToFlowDataSet": {"shortDescription": [{"value": "Welded and zinc coated steel structures (Heidelberg Materials SBC Latvia SIA)", "lang": "en"}], "type": "flow data set", "refObjectId": "c8372ddc-ebc5-49a9-bb70-d4be92f03610", "version": "00.00.002"}, "meanAmount": 1.0, "resultingAmount": 1.0, "referenceFlow": true, "resultingflowAmount": 1000.0, "flowProperties": [{"name": [{"lang": "en", "value": "Mass"}, {"lang": "de", "value": "Masse"}], "uuid": "93a60a56-a3c8-11da-a746-0800200b9a66", "referenceFlowProperty": true, "meanValue": 1000.0, "referenceUnit": "kg", "unitGroupUUID": "ad38d542-3fe9-439d-9b95-2f5f7752acaf"}], "materialProperties": [{"name": "gross density", "value": "7850.0", "unit": "kg/m^3", "unitDescription": "kilograms per cubic metre"}], "typeOfFlow": "Product flow", "classification": {"classHierarchy": "Metalle / Stahl und Eisen / Stahlprofile", "name": "OEKOBAU.DAT"}}, {"dataSetInternalID": 2, "referenceToFlowDataSet": {"shortDescription": [{"value": "Components for re-use (CRU)", "lang": "en"}, {"value": "Komponenten für die Wiederverwendung (CRU)", "lang": "de"}, {"value": "Componentes para su reutilización (CRU)", "lang": "es"}], "type": "flow data set", "refObjectId": "a2b32f97-3fc7-4af2-b209-525bc6426f33", "version": "30.00.000", "uri": "../flows/a2b32f97-3fc7-4af2-b209-525bc6426f33.xml"}, "exchange direction": "OUTPUT", "meanAmount": 0.0, "other": {"anies": [{"value": "0.0", "module": "A1", "scenario": "Standard Scenario"}, {"value": "0.0", "module": "A2", "scenario": "Standard Scenario"}, {"value": "0.0", "module": "A3", "scenario": "Standard Scenario"}, {"value": "0.0", "module": "A4", "scenario": "Norway Scenario"}, {"value": "0.0", "module": "A4", "scenario": "Sweden Scenario"}, {"value": "0.0", "module": "C1", "scenario": "Standard Scenario"}, {"value": "0.0", "module": "C2", "scenario": "Standard Scenario"}, {"value": "0.0", "module": "C3", "scenario": "Standard Scenario"}, {"value": "0.0", "module": "C4", "scenario": "Standard Scenario"}, {"value": "0.0", "module": "D", "scenario": "Standard Scenario"}, {"name": "referenceToUnitGroupDataSet", "value": {"shortDescription": [{"value": "kg", "lang": "en"}], "type": "unit group data set", "refObjectId": "ad38d542-3fe9-439d-9b95-2f5f7752acaf", "version": "30.00.000", "uri": "../unitgroups/ad38d542-3fe9-439d-9b95-2f5f7752acaf.xml"}}]}, "flowProperties": [], "typeOfFlow": "Other flow", "classification": {"classHierarchy": "Größen / Umweltliche Größen / EPD EN 15804 / LCI Indikatoren", "name": "GaBiCategories"}}, {"dataSetInternalID": 3, "referenceToFlowDataSet": {"shortDescription": [{"value": "Exported electrical energy (EEE)", "lang": "en"}, {"value": "Exportierte elektrische Energie (EEE)", "lang": "de"}, {"value": "Energía exportada electrica (EEE)", "lang": "es"}], "type": "flow data set", "refObjectId": "4da0c987-2b76-40d6-9e9e-82a017aaaf29", "version": "30.00.000", "uri": "../flows/4da0c987-2b76-40d6-9e9e-82a017aaaf29.xml"}, "exchange direction": "OUTPUT", "meanAmount": 0.0, "other": {"anies": [{"value": "0.0", "module": "A1", "scenario": "Standard Scenario"}, {"value": "0.0", "module": "A2", "scenario": "Standard Scenario"}, {"value": "0.0", "module": "A3", "scenario": "Standard Scenario"}, {"value": "0.0", "module": "A4", "scenario": "Norway Scenario"}, {"value": "0.0", "module": "A4", "scenario": "Sweden Scenario"}, {"value": "0.0", "module": "C1", "scenario": "Standard Scenario"}, {"value": "0.0", "module": "C2", "scenario": "Standard Scenario"}, {"value": "0.0", "module": "C3", "scenario": "Standard Scenario"}, {"value": "0.0", "module": "C4", "scenario": "Standard Scenario"}, {"value": "25.1", "module": "D", "scenario": "Standard Scenario"}, {"name": "referenceToUnitGroupDataSet", "value": {"shortDescription": [{"value": "MJ", "lang": "en"}], "type": "unit group data set", "refObjectId": "93a60a57-a3c8-11da-a746-0800200c9a66", "version": "03.00.000", "uri": "../unitgroups/93a60a57-a3c8-11da-a746-0800200c9a66.xml"}}]}, "flowProperties": [], "typeOfFlow": "Other flow", "classification": {"classHierarchy": "Größen / Umweltliche Größen / EPD EN 15804 / LCI Indikatoren", "name": "GaBiCategories"}}, {"dataSetInternalID": 4, "referenceToFlowDataSet": {"shortDescription": [{"value": "Exported thermal energy (EET)", "lang": "en"}, {"value": "Exportierte thermische Energie (EET)", "lang": "de"}, {"value": "Energía exportada termal (EET)", "lang": "es"}], "type": "flow data set", "refObjectId": "98daf38a-7a79-46d3-9a37-2b7bd0955810", "version": "30.00.000", "uri": "../flows/98daf38a-7a79-46d3-9a37-2b7bd0955810.xml"}, "exchange direction": "OUTPUT", "meanAmount": 0.0, "other": {"anies": [{"value": "0.0", "module": "A1", "scenario": "Standard Scenario"}, {"value": "0.0", "module": "A2", "scenario": "Standard Scenario"}, {"value": "0.0", "module": "A3", "scenario": "Standard Scenario"}, {"value": "0.0", "module": "A4", "scenario": "Norway Scenario"}, {"value": "0.0", "module": "A4", "scenario": "Sweden Scenario"}, {"value": "0.0", "module": "C1", "scenario": "Standard Scenario"}, {"value": "0.0", "module": "C2", "scenario": "Standard Scenario"}, {"value": "0.0", "module": "C3", "scenario": "Standard Scenario"}, {"value": "0.0", "module": "C4", "scenario": "Standard Scenario"}, {"value": "43.2", "module": "D", "scenario": "Standard Scenario"}, {"name": "referenceToUnitGroupDataSet", "value": {"shortDescription": [{"value": "MJ", "lang": "en"}], "type": "unit group data set", "refObjectId": "93a60a57-a3c8-11da-a746-0800200c9a66", "version": "03.00.000", "uri": "../unitgroups/93a60a57-a3c8-11da-a746-0800200c9a66.xml"}}]}, "flowProperties": [], "typeOfFlow": "Other flow", "classification": {"classHierarchy": "Größen / Umweltliche Größen / EPD EN 15804 / LCI Indikatoren", "name": "GaBiCategories"}}, {"dataSetInternalID": 5, "referenceToFlowDataSet": {"shortDescription": [{"value": "Use of net fresh water (FW)", "lang": "en"}, {"value": "Einsatz von Süßwasserressourcen (FW)", "lang": "de"}, {"value": "Uso neto de recursos de agua dulce (FW)", "lang": "es"}], "type": "flow data set", "refObjectId": "3cf952c8-f3a4-461d-8c96-96456ca62246", "version": "30.00.000", "uri": "../flows/3cf952c8-f3a4-461d-8c96-96456ca62246.xml"}, "exchange direction": "INPUT", "meanAmount": 0.0, "other": {"anies": [{"value": "21.4", "module": "A1", "scenario": "Standard Scenario"}, {"value": "0.339", "module": "A2", "scenario": "Standard Scenario"}, {"value": "13.2", "module": "A3", "scenario": "Standard Scenario"}, {"value": "0.202", "module": "A4", "scenario": "Norway Scenario"}, {"value": "0.0713", "module": "A4", "scenario": "Sweden Scenario"}, {"value": "0.00256", "module": "C1", "scenario": "Standard Scenario"}, {"value": "0.013", "module": "C2", "scenario": "Standard Scenario"}, {"value": "0.0647", "module": "C3", "scenario": "Standard Scenario"}, {"value": "0.015", "module": "C4", "scenario": "Standard Scenario"}, {"value": "0.0465", "module": "D", "scenario": "Standard Scenario"}, {"name": "referenceToUnitGroupDataSet", "value": {"shortDescription": [{"value": "m3", "lang": "en"}], "type": "unit group data set", "refObjectId": "cd950537-0a98-4044-9ba7-9f9a68d0a504", "version": "30.00.000", "uri": "../unitgroups/cd950537-0a98-4044-9ba7-9f9a68d0a504.xml"}}]}, "flowProperties": [], "typeOfFlow": "Other flow", "classification": {"classHierarchy": "Größen / Umweltliche Größen / EPD EN 15804 / LCI Indikatoren", "name": "GaBiCategories"}}, {"dataSetInternalID": 6, "referenceToFlowDataSet": {"shortDescription": [{"value": "Hazardous waste disposed (HWD)", "lang": "en"}, {"value": "Gefährlicher Abfall zur Deponie (HWD)", "lang": "de"}, {"value": "Residuos peligrosos eliminados (HWD)", "lang": "es"}], "type": "flow data set", "refObjectId": "430f9e0f-59b2-46a0-8e0d-55e0e84948fc", "version": "30.00.000", "uri": "../flows/430f9e0f-59b2-46a0-8e0d-55e0e84948fc.xml"}, "exchange direction": "OUTPUT", "meanAmount": 0.0, "other": {"anies": [{"value": "0.0581", "module": "A1", "scenario": "Standard Scenario"}, {"value": "0.00851", "module": "A2", "scenario": "Standard Scenario"}, {"value": "0.964", "module": "A3", "scenario": "Standard Scenario"}, {"value": "0.00494", "module": "A4", "scenario": "Norway Scenario"}, {"value": "0.00173", "module": "A4", "scenario": "Sweden Scenario"}, {"value": "1.35E-4", "module": "C1", "scenario": "Standard Scenario"}, {"value": "2.71E-4", "module": "C2", "scenario": "Standard Scenario"}, {"value": "0.00207", "module": "C3", "scenario": "Standard Scenario"}, {"value": "1.48E-5", "module": "C4", "scenario": "Standard Scenario"}, {"value": "0.00159", "module": "D", "scenario": "Standard Scenario"}, {"name": "referenceToUnitGroupDataSet", "value": {"shortDescription": [{"value": "kg", "lang": "en"}], "type": "unit group data set", "refObjectId": "ad38d542-3fe9-439d-9b95-2f5f7752acaf", "version": "30.00.000", "uri": "../unitgroups/ad38d542-3fe9-439d-9b95-2f5f7752acaf.xml"}}]}, "flowProperties": [], "typeOfFlow": "Other flow", "classification": {"classHierarchy": "Größen / Umweltliche Größen / EPD EN 15804 / LCI Indikatoren", "name": "GaBiCategories"}}, {"dataSetInternalID": 7, "referenceToFlowDataSet": {"shortDescription": [{"value": "Materials for energy recovery (MER)", "lang": "en"}, {"value": "Stoffe für die Energierückgewinnung (MER)", "lang": "de"}, {"value": "Materiales para valorización energética (recuperación de energía) (MER)", "lang": "es"}], "type": "flow data set", "refObjectId": "59a9181c-3aaf-46ee-8b13-2b3723b6e447", "version": "30.00.000", "uri": "../flows/59a9181c-3aaf-46ee-8b13-2b3723b6e447.xml"}, "exchange direction": "OUTPUT", "meanAmount": 0.0, "other": {"anies": [{"value": "0.0", "module": "A1", "scenario": "Standard Scenario"}, {"value": "0.0", "module": "A2", "scenario": "Standard Scenario"}, {"value": "0.0", "module": "A3", "scenario": "Standard Scenario"}, {"value": "0.0", "module": "A4", "scenario": "Norway Scenario"}, {"value": "0.0", "module": "A4", "scenario": "Sweden Scenario"}, {"value": "0.0", "module": "C1", "scenario": "Standard Scenario"}, {"value": "0.0", "module": "C2", "scenario": "Standard Scenario"}, {"value": "0.0", "module": "C3", "scenario": "Standard Scenario"}, {"value": "0.0", "module": "C4", "scenario": "Standard Scenario"}, {"value": "0.0", "module": "D", "scenario": "Standard Scenario"}, {"name": "referenceToUnitGroupDataSet", "value": {"shortDescription": [{"value": "kg", "lang": "en"}], "type": "unit group data set", "refObjectId": "ad38d542-3fe9-439d-9b95-2f5f7752acaf", "version": "30.00.000", "uri": "../unitgroups/ad38d542-3fe9-439d-9b95-2f5f7752acaf.xml"}}]}, "flowProperties": [], "typeOfFlow": "Other flow", "classification": {"classHierarchy": "Größen / Umweltliche Größen / EPD EN 15804 / LCI Indikatoren", "name": "GaBiCategories"}}, {"dataSetInternalID": 8, "referenceToFlowDataSet": {"shortDescription": [{"value": "Materials for recycling (MFR)", "lang": "en"}, {"value": "Stoffe zum Recycling (MFR)", "lang": "de"}, {"value": "Materiales para el reciclaje (MFR)", "lang": "es"}], "type": "flow data set", "refObjectId": "d7fe48a5-4103-49c8-9aae-b0b5dfdbd6ae", "version": "30.00.000", "uri": "../flows/d7fe48a5-4103-49c8-9aae-b0b5dfdbd6ae.xml"}, "exchange direction": "OUTPUT", "meanAmount": 0.0, "other": {"anies": [{"value": "0.0", "module": "A1", "scenario": "Standard Scenario"}, {"value": "0.0", "module": "A2", "scenario": "Standard Scenario"}, {"value": "58.6", "module": "A3", "scenario": "Standard Scenario"}, {"value": "0.0", "module": "A4", "scenario": "Norway Scenario"}, {"value": "0.0", "module": "A4", "scenario": "Sweden Scenario"}, {"value": "0.0", "module": "C1", "scenario": "Standard Scenario"}, {"value": "0.0", "module": "C2", "scenario": "Standard Scenario"}, {"value": "0.0", "module": "C3", "scenario": "Standard Scenario"}, {"value": "0.0", "module": "C4", "scenario": "Standard Scenario"}, {"value": "0.0", "module": "D", "scenario": "Standard Scenario"}, {"name": "referenceToUnitGroupDataSet", "value": {"shortDescription": [{"value": "kg", "lang": "en"}], "type": "unit group data set", "refObjectId": "ad38d542-3fe9-439d-9b95-2f5f7752acaf", "version": "30.00.000", "uri": "../unitgroups/ad38d542-3fe9-439d-9b95-2f5f7752acaf.xml"}}]}, "flowProperties": [], "typeOfFlow": "Other flow", "classification": {"classHierarchy": "Größen / Umweltliche Größen / EPD EN 15804 / LCI Indikatoren", "name": "GaBiCategories"}}, {"dataSetInternalID": 9, "referenceToFlowDataSet": {"shortDescription": [{"value": "Non-hazardous waste disposed (NHWD)", "lang": "en"}, {"value": "Entsorgter nicht gefährlicher Abfall (NHWD)", "lang": "de"}, {"value": "Residuos no peligrosos eliminados (NHWD)", "lang": "es"}], "type": "flow data set", "refObjectId": "b29ef66b-e286-4afa-949f-62f1a7b4d7fa", "version": "30.00.000", "uri": "../flows/b29ef66b-e286-4afa-949f-62f1a7b4d7fa.xml"}, "exchange direction": "OUTPUT", "meanAmount": 0.0, "other": {"anies": [{"value": "458.0", "module": "A1", "scenario": "Standard Scenario"}, {"value": "154.0", "module": "A2", "scenario": "Standard Scenario"}, {"value": "128.0", "module": "A3", "scenario": "Standard Scenario"}, {"value": "91.2", "module": "A4", "scenario": "Norway Scenario"}, {"value": "31.7", "module": "A4", "scenario": "Sweden Scenario"}, {"value": "0.0588", "module": "C1", "scenario": "Standard Scenario"}, {"value": "6.78", "module": "C2", "scenario": "Standard Scenario"}, {"value": "1.0", "module": "C3", "scenario": "Standard Scenario"}, {"value": "50.1", "module": "C4", "scenario": "Standard Scenario"}, {"value": "1.04", "module": "D", "scenario": "Standard Scenario"}, {"name": "referenceToUnitGroupDataSet", "value": {"shortDescription": [{"value": "kg", "lang": "en"}], "type": "unit group data set", "refObjectId": "ad38d542-3fe9-439d-9b95-2f5f7752acaf", "version": "30.00.000", "uri": "../unitgroups/ad38d542-3fe9-439d-9b95-2f5f7752acaf.xml"}}]}, "flowProperties": [], "typeOfFlow": "Other flow", "classification": {"classHierarchy": "Größen / Umweltliche Größen / EPD EN 15804 / LCI Indikatoren", "name": "GaBiCategories"}}, {"dataSetInternalID": 10, "referenceToFlowDataSet": {"shortDescription": [{"value": "Use of non renewable secondary fuels (NRSF)", "lang": "en"}, {"value": "Nicht erneuerbare Sekundärbrennstoffe (NRSF)", "lang": "de"}, {"value": "Uso de combustibles secundarios no renovables (NRSF)", "lang": "es"}], "type": "flow data set", "refObjectId": "89def144-d39a-4287-b86f-efde453ddcb2", "version": "30.00.000", "uri": "../flows/89def144-d39a-4287-b86f-efde453ddcb2.xml"}, "exchange direction": "INPUT", "meanAmount": 0.0, "other": {"anies": [{"value": "0.0", "module": "A1", "scenario": "Standard Scenario"}, {"value": "0.0", "module": "A2", "scenario": "Standard Scenario"}, {"value": "236.0", "module": "A3", "scenario": "Standard Scenario"}, {"value": "0.0", "module": "A4", "scenario": "Norway Scenario"}, {"value": "0.0", "module": "A4", "scenario": "Sweden Scenario"}, {"value": "0.0", "module": "C1", "scenario": "Standard Scenario"}, {"value": "0.0", "module": "C2", "scenario": "Standard Scenario"}, {"value": "0.0", "module": "C3", "scenario": "Standard Scenario"}, {"value": "0.0", "module": "C4", "scenario": "Standard Scenario"}, {"value": "0.0", "module": "D", "scenario": "Standard Scenario"}, {"name": "referenceToUnitGroupDataSet", "value": {"shortDescription": [{"value": "MJ", "lang": "en"}], "type": "unit group data set", "refObjectId": "93a60a57-a3c8-11da-a746-0800200c9a66", "version": "03.00.000", "uri": "../unitgroups/93a60a57-a3c8-11da-a746-0800200c9a66.xml"}}]}, "flowProperties": [], "typeOfFlow": "Other flow", "classification": {"classHierarchy": "Größen / Umweltliche Größen / EPD EN 15804 / LCI Indikatoren", "name": "GaBiCategories"}}, {"dataSetInternalID": 11, "referenceToFlowDataSet": {"shortDescription": [{"value": "Use of non renewable primary energy (PENRE)", "lang": "en"}, {"value": "Nicht-erneuerbare Primärenergie als Energieträger (PENRE)", "lang": "de"}, {"value": "Uso de energía primaria no renovable, excluyendo los recursos de energía primaria no renovable utilizada como materia prima (PENRE)", "lang": "es"}], "type": "flow data set", "refObjectId": "ac857178-2b45-46ec-892a-a9a4332f0372", "version": "38.00.000", "uri": "../flows/ac857178-2b45-46ec-892a-a9a4332f0372.xml"}, "exchange direction": "INPUT", "meanAmount": 0.0, "other": {"anies": [{"value": "18500.0", "module": "A1", "scenario": "Standard Scenario"}, {"value": "3420.0", "module": "A2", "scenario": "Standard Scenario"}, {"value": "10100.0", "module": "A3", "scenario": "Standard Scenario"}, {"value": "2030.0", "module": "A4", "scenario": "Norway Scenario"}, {"value": "726.0", "module": "A4", "scenario": "Sweden Scenario"}, {"value": "52.7", "module": "C1", "scenario": "Standard Scenario"}, {"value": "113.0", "module": "C2", "scenario": "Standard Scenario"}, {"value": "830.0", "module": "C3", "scenario": "Standard Scenario"}, {"value": "12.7", "module": "C4", "scenario": "Standard Scenario"}, {"value": "89.2", "module": "D", "scenario": "Standard Scenario"}, {"name": "referenceToUnitGroupDataSet", "value": {"shortDescription": [{"value": "MJ", "lang": "en"}], "type": "unit group data set", "refObjectId": "93a60a57-a3c8-11da-a746-0800200c9a66", "version": "03.00.000", "uri": "../unitgroups/93a60a57-a3c8-11da-a746-0800200c9a66.xml"}}]}, "flowProperties": [], "typeOfFlow": "Other flow", "classification": {"classHierarchy": "Quantities", "name": "GaBiCategories"}}, {"dataSetInternalID": 12, "referenceToFlowDataSet": {"shortDescription": [{"value": "Use of non renewable primary energy resources used as raw materials (PENRM)", "lang": "en"}, {"value": "Nicht-erneuerbare Primärenergie zur stofflichen Nutzung (PENRM)", "lang": "de"}, {"value": "Uso de la energía primaria no renovable utilizada como materia prima (PENRM)", "lang": "es"}], "type": "flow data set", "refObjectId": "1421caa0-679d-4bf4-b282-0eb850ccae27", "version": "38.00.000", "uri": "../flows/1421caa0-679d-4bf4-b282-0eb850ccae27.xml"}, "exchange direction": "INPUT", "meanAmount": 0.0, "other": {"anies": [{"value": "0.0", "module": "A1", "scenario": "Standard Scenario"}, {"value": "0.0", "module": "A2", "scenario": "Standard Scenario"}, {"value": "2.77", "module": "A3", "scenario": "Standard Scenario"}, {"value": "0.0", "module": "A4", "scenario": "Norway Scenario"}, {"value": "0.0", "module": "A4", "scenario": "Sweden Scenario"}, {"value": "0.0", "module": "C1", "scenario": "Standard Scenario"}, {"value": "0.0", "module": "C2", "scenario": "Standard Scenario"}, {"value": "0.0", "module": "C3", "scenario": "Standard Scenario"}, {"value": "0.0", "module": "C4", "scenario": "Standard Scenario"}, {"value": "0.0", "module": "D", "scenario": "Standard Scenario"}, {"name": "referenceToUnitGroupDataSet", "value": {"shortDescription": [{"value": "MJ", "lang": "en"}], "type": "unit group data set", "refObjectId": "93a60a57-a3c8-11da-a746-0800200c9a66", "version": "03.00.000", "uri": "../unitgroups/93a60a57-a3c8-11da-a746-0800200c9a66.xml"}}]}, "flowProperties": [], "typeOfFlow": "Other flow", "classification": {"classHierarchy": "Quantities", "name": "GaBiCategories"}}, {"dataSetInternalID": 13, "referenceToFlowDataSet": {"shortDescription": [{"value": "Total use of non-renewable primary energy resources (PENRT)", "lang": "en"}, {"value": "Total nicht erneuerbare Primärenergie (PENRT)", "lang": "de"}, {"value": "Uso total de la energía primaria no renovable (energía primaria y recursos de energía primaria renovable utilizada como materia prima) (PENRT)", "lang": "es"}], "type": "flow data set", "refObjectId": "06159210-646b-4c8d-8583-da9b3b95a6c1", "version": "30.00.000", "uri": "../flows/06159210-646b-4c8d-8583-da9b3b95a6c1.xml"}, "exchange direction": "INPUT", "meanAmount": 0.0, "other": {"anies": [{"value": "18500.0", "module": "A1", "scenario": "Standard Scenario"}, {"value": "3420.0", "module": "A2", "scenario": "Standard Scenario"}, {"value": "10100.0", "module": "A3", "scenario": "Standard Scenario"}, {"value": "2030.0", "module": "A4", "scenario": "Norway Scenario"}, {"value": "726.0", "module": "A4", "scenario": "Sweden Scenario"}, {"value": "52.7", "module": "C1", "scenario": "Standard Scenario"}, {"value": "113.0", "module": "C2", "scenario": "Standard Scenario"}, {"value": "830.0", "module": "C3", "scenario": "Standard Scenario"}, {"value": "12.7", "module": "C4", "scenario": "Standard Scenario"}, {"value": "89.2", "module": "D", "scenario": "Standard Scenario"}, {"name": "referenceToUnitGroupDataSet", "value": {"shortDescription": [{"value": "MJ", "lang": "en"}], "type": "unit group data set", "refObjectId": "93a60a57-a3c8-11da-a746-0800200c9a66", "version": "03.00.000", "uri": "../unitgroups/93a60a57-a3c8-11da-a746-0800200c9a66.xml"}}]}, "flowProperties": [], "typeOfFlow": "Other flow", "classification": {"classHierarchy": "Größen / Umweltliche Größen / EPD EN 15804 / LCI Indikatoren", "name": "GaBiCategories"}}, {"dataSetInternalID": 14, "referenceToFlowDataSet": {"shortDescription": [{"value": "Use of renewable primary energy (PERE)", "lang": "en"}, {"value": "Erneuerbare Primärenergie als Energieträger (PERE)", "lang": "de"}, {"value": "Uso de energía primaria renovable excluyendo los recursos de energía primaria renovable utilizada como materia prima (PERE)", "lang": "es"}], "type": "flow data set", "refObjectId": "20f32be5-0398-4288-9b6d-accddd195317", "version": "38.00.000", "uri": "../flows/20f32be5-0398-4288-9b6d-accddd195317.xml"}, "exchange direction": "INPUT", "meanAmount": 0.0, "other": {"anies": [{"value": "1630.0", "module": "A1", "scenario": "Standard Scenario"}, {"value": "45.5", "module": "A2", "scenario": "Standard Scenario"}, {"value": "1760.0", "module": "A3", "scenario": "Standard Scenario"}, {"value": "27.0", "module": "A4", "scenario": "Norway Scenario"}, {"value": "9.53", "module": "A4", "scenario": "Sweden Scenario"}, {"value": "0.268", "module": "C1", "scenario": "Standard Scenario"}, {"value": "1.34", "module": "C2", "scenario": "Standard Scenario"}, {"value": "9.96", "module": "C3", "scenario": "Standard Scenario"}, {"value": "0.677", "module": "C4", "scenario": "Standard Scenario"}, {"value": "-158.0", "module": "D", "scenario": "Standard Scenario"}, {"name": "referenceToUnitGroupDataSet", "value": {"shortDescription": [{"value": "MJ", "lang": "en"}], "type": "unit group data set", "refObjectId": "93a60a57-a3c8-11da-a746-0800200c9a66", "version": "03.00.000", "uri": "../unitgroups/93a60a57-a3c8-11da-a746-0800200c9a66.xml"}}]}, "flowProperties": [], "typeOfFlow": "Other flow", "classification": {"classHierarchy": "Quantities", "name": "GaBiCategories"}}, {"dataSetInternalID": 15, "referenceToFlowDataSet": {"shortDescription": [{"value": "Use of renewable primary energy resources used as raw materials (PERM)", "lang": "en"}, {"value": "Erneuerbare Primärenergie zur stofflichen Nutzung (PERM)", "lang": "de"}, {"value": "Uso de energía primaria renovable utilizada como materia prima (PERM)", "lang": "es"}], "type": "flow data set", "refObjectId": "fb3ec0de-548d-4508-aea5-00b73bf6f702", "version": "38.00.000", "uri": "../flows/fb3ec0de-548d-4508-aea5-00b73bf6f702.xml"}, "exchange direction": "INPUT", "meanAmount": 0.0, "other": {"anies": [{"value": "0.0", "module": "A1", "scenario": "Standard Scenario"}, {"value": "0.0", "module": "A2", "scenario": "Standard Scenario"}, {"value": "159.0", "module": "A3", "scenario": "Standard Scenario"}, {"value": "0.0", "module": "A4", "scenario": "Norway Scenario"}, {"value": "0.0", "module": "A4", "scenario": "Sweden Scenario"}, {"value": "0.0", "module": "C1", "scenario": "Standard Scenario"}, {"value": "0.0", "module": "C2", "scenario": "Standard Scenario"}, {"value": "0.0", "module": "C3", "scenario": "Standard Scenario"}, {"value": "0.0", "module": "C4", "scenario": "Standard Scenario"}, {"value": "0.0", "module": "D", "scenario": "Standard Scenario"}, {"name": "referenceToUnitGroupDataSet", "value": {"shortDescription": [{"value": "MJ", "lang": "en"}], "type": "unit group data set", "refObjectId": "93a60a57-a3c8-11da-a746-0800200c9a66", "version": "03.00.000", "uri": "../unitgroups/93a60a57-a3c8-11da-a746-0800200c9a66.xml"}}]}, "flowProperties": [], "typeOfFlow": "Other flow", "classification": {"classHierarchy": "Quantities", "name": "GaBiCategories"}}, {"dataSetInternalID": 16, "referenceToFlowDataSet": {"shortDescription": [{"value": "Total use of renewable primary energy resources (PERT)", "lang": "en"}, {"value": "Total erneuerbare Primärenergie (PERT)", "lang": "de"}, {"value": "Uso total de la energía primaria renovable (energía primaria y recursos de energía primaria renovable utilizada como materia prima) (PERT)", "lang": "es"}], "type": "flow data set", "refObjectId": "53f97275-fa8a-4cdd-9024-65936002acd0", "version": "30.00.000", "uri": "../flows/53f97275-fa8a-4cdd-9024-65936002acd0.xml"}, "exchange direction": "INPUT", "meanAmount": 0.0, "other": {"anies": [{"value": "1630.0", "module": "A1", "scenario": "Standard Scenario"}, {"value": "45.5", "module": "A2", "scenario": "Standard Scenario"}, {"value": "1920.0", "module": "A3", "scenario": "Standard Scenario"}, {"value": "27.0", "module": "A4", "scenario": "Norway Scenario"}, {"value": "9.53", "module": "A4", "scenario": "Sweden Scenario"}, {"value": "0.268", "module": "C1", "scenario": "Standard Scenario"}, {"value": "1.34", "module": "C2", "scenario": "Standard Scenario"}, {"value": "9.96", "module": "C3", "scenario": "Standard Scenario"}, {"value": "0.677", "module": "C4", "scenario": "Standard Scenario"}, {"value": "-158.0", "module": "D", "scenario": "Standard Scenario"}, {"name": "referenceToUnitGroupDataSet", "value": {"shortDescription": [{"value": "MJ", "lang": "en"}], "type": "unit group data set", "refObjectId": "93a60a57-a3c8-11da-a746-0800200c9a66", "version": "03.00.000", "uri": "../unitgroups/93a60a57-a3c8-11da-a746-0800200c9a66.xml"}}]}, "flowProperties": [], "typeOfFlow": "Other flow", "classification": {"classHierarchy": "Größen / Umweltliche Größen / EPD EN 15804 / LCI Indikatoren", "name": "GaBiCategories"}}, {"dataSetInternalID": 17, "referenceToFlowDataSet": {"shortDescription": [{"value": "Use of renewable secondary fuels (RSF)", "lang": "en"}, {"value": "Erneuerbare Sekundärbrennstoffe (RSF)", "lang": "de"}, {"value": "Uso de combustibles secundarios renovables (RSF)", "lang": "es"}], "type": "flow data set", "refObjectId": "64333088-a55f-4aa2-9a31-c10b07816787", "version": "30.00.000", "uri": "../flows/64333088-a55f-4aa2-9a31-c10b07816787.xml"}, "exchange direction": "INPUT", "meanAmount": 0.0, "other": {"anies": [{"value": "0.0", "module": "A1", "scenario": "Standard Scenario"}, {"value": "0.0", "module": "A2", "scenario": "Standard Scenario"}, {"value": "0.0", "module": "A3", "scenario": "Standard Scenario"}, {"value": "0.0", "module": "A4", "scenario": "Norway Scenario"}, {"value": "0.0", "module": "A4", "scenario": "Sweden Scenario"}, {"value": "0.0", "module": "C1", "scenario": "Standard Scenario"}, {"value": "0.0", "module": "C2", "scenario": "Standard Scenario"}, {"value": "0.0", "module": "C3", "scenario": "Standard Scenario"}, {"value": "0.0", "module": "C4", "scenario": "Standard Scenario"}, {"value": "0.0", "module": "D", "scenario": "Standard Scenario"}, {"name": "referenceToUnitGroupDataSet", "value": {"shortDescription": [{"value": "MJ", "lang": "en"}], "type": "unit group data set", "refObjectId": "93a60a57-a3c8-11da-a746-0800200c9a66", "version": "03.00.000", "uri": "../unitgroups/93a60a57-a3c8-11da-a746-0800200c9a66.xml"}}]}, "flowProperties": [], "typeOfFlow": "Other flow", "classification": {"classHierarchy": "Größen / Umweltliche Größen / EPD EN 15804 / LCI Indikatoren", "name": "GaBiCategories"}}, {"dataSetInternalID": 18, "referenceToFlowDataSet": {"shortDescription": [{"value": "Radioactive waste disposed (RWD)", "lang": "en"}, {"value": "Entsorgter radioaktiver Abfall (RWD)", "lang": "de"}, {"value": "Residuos radiactivos eliminados (RWD)", "lang": "es"}], "type": "flow data set", "refObjectId": "3449546e-52ad-4b39-b809-9fb77cea8ff6", "version": "30.00.000", "uri": "../flows/3449546e-52ad-4b39-b809-9fb77cea8ff6.xml"}, "exchange direction": "OUTPUT", "meanAmount": 0.0, "other": {"anies": [{"value": "0.0623", "module": "A1", "scenario": "Standard Scenario"}, {"value": "0.0219", "module": "A2", "scenario": "Standard Scenario"}, {"value": "0.0418", "module": "A3", "scenario": "Standard Scenario"}, {"value": "0.013", "module": "A4", "scenario": "Norway Scenario"}, {"value": "0.00466", "module": "A4", "scenario": "Sweden Scenario"}, {"value": "3.45E-4", "module": "C1", "scenario": "Standard Scenario"}, {"value": "7.02E-4", "module": "C2", "scenario": "Standard Scenario"}, {"value": "0.00543", "module": "C3", "scenario": "Standard Scenario"}, {"value": "7.93E-5", "module": "C4", "scenario": "Standard Scenario"}, {"value": "-1.28E-4", "module": "D", "scenario": "Standard Scenario"}, {"name": "referenceToUnitGroupDataSet", "value": {"shortDescription": [{"value": "kg", "lang": "en"}], "type": "unit group data set", "refObjectId": "ad38d542-3fe9-439d-9b95-2f5f7752acaf", "version": "30.00.000", "uri": "../unitgroups/ad38d542-3fe9-439d-9b95-2f5f7752acaf.xml"}}]}, "flowProperties": [], "typeOfFlow": "Other flow", "classification": {"classHierarchy": "Größen / Umweltliche Größen / EPD EN 15804 / LCI Indikatoren", "name": "GaBiCategories"}}, {"dataSetInternalID": 19, "referenceToFlowDataSet": {"shortDescription": [{"value": "Use of secondary material (SM)", "lang": "en"}, {"value": "Einsatz von Sekundärstoffen (SM)", "lang": "de"}, {"value": "Uso de materiales secundarios (SM)", "lang": "es"}], "type": "flow data set", "refObjectId": "c6a1f35f-2d09-4f54-8dfb-97e502e1ce92", "version": "30.00.000", "uri": "../flows/c6a1f35f-2d09-4f54-8dfb-97e502e1ce92.xml"}, "exchange direction": "INPUT", "meanAmount": 0.0, "other": {"anies": [{"value": "755.0", "module": "A1", "scenario": "Standard Scenario"}, {"value": "0.0", "module": "A2", "scenario": "Standard Scenario"}, {"value": "47.3", "module": "A3", "scenario": "Standard Scenario"}, {"value": "0.0", "module": "A4", "scenario": "Norway Scenario"}, {"value": "0.0", "module": "A4", "scenario": "Sweden Scenario"}, {"value": "0.0", "module": "C1", "scenario": "Standard Scenario"}, {"value": "0.0", "module": "C2", "scenario": "Standard Scenario"}, {"value": "950.0", "module": "C3", "scenario": "Standard Scenario"}, {"value": "0.0", "module": "C4", "scenario": "Standard Scenario"}, {"value": "0.0", "module": "D", "scenario": "Standard Scenario"}, {"name": "referenceToUnitGroupDataSet", "value": {"shortDescription": [{"value": "kg", "lang": "en"}], "type": "unit group data set", "refObjectId": "ad38d542-3fe9-439d-9b95-2f5f7752acaf", "version": "30.00.000", "uri": "../unitgroups/ad38d542-3fe9-439d-9b95-2f5f7752acaf.xml"}}]}, "flowProperties": [], "typeOfFlow": "Other flow", "classification": {"classHierarchy": "Größen / Umweltliche Größen / EPD EN 15804 / LCI Indikatoren", "name": "GaBiCategories"}}]}, "LCIAResults": {"LCIAResult": [{"referenceToLCIAMethodDataSet": {"shortDescription": [{"value": "Abiotic depletion potential - non-fossil resources (ADPE)", "lang": "en"}, {"value": "Potenzial für die Verknappung abiotischer Ressourcen – nicht fossile Ressourcen (ADPE)", "lang": "de"}], "type": "LCIA method data set", "refObjectId": "b2ad6494-c78d-11e6-9d9d-cec0c932ce01", "version": "01.00.011", "uri": "../lciamethods/b2ad6494-c78d-11e6-9d9d-cec0c932ce01.xml"}, "meanAmount": 0.0, "other": {"anies": [{"value": "0.0171", "module": "A1", "scenario": "Standard Scenario"}, {"value": "0.00577", "module": "A2", "scenario": "Standard Scenario"}, {"value": "7.52", "module": "A3", "scenario": "Standard Scenario"}, {"value": "0.00344", "module": "A4", "scenario": "Norway Scenario"}, {"value": "0.00121", "module": "A4", "scenario": "Sweden Scenario"}, {"value": "5.53E-6", "module": "C1", "scenario": "Standard Scenario"}, {"value": "1.8E-4", "module": "C2", "scenario": "Standard Scenario"}, {"value": "9.51E-5", "module": "C3", "scenario": "Standard Scenario"}, {"value": "3.94E-6", "module": "C4", "scenario": "Standard Scenario"}, {"value": "-6.11E-8", "module": "D", "scenario": "Standard Scenario"}, {"name": "referenceToUnitGroupDataSet", "value": {"shortDescription": [{"value": "kg Sb-eq.", "lang": "en"}], "type": "unit group data set", "refObjectId": "54ccd2d9-a32a-4fc2-923d-f2c8c93e89d4", "version": "30.00.000", "uri": "../unitgroups/54ccd2d9-a32a-4fc2-923d-f2c8c93e89d4.xml"}}]}}, {"referenceToLCIAMethodDataSet": {"shortDescription": [{"value": "Abiotic depletion potential - fossil resources (ADPF)", "lang": "en"}, {"value": "Potenzial für die Verknappung abiotischer Ressourcen – fossile Brennstoffe (ADPF)", "lang": "de"}], "type": "LCIA method data set", "refObjectId": "b2ad6110-c78d-11e6-9d9d-cec0c932ce01", "version": "01.00.011", "uri": "../lciamethods/b2ad6110-c78d-11e6-9d9d-cec0c932ce01.xml"}, "meanAmount": 0.0, "other": {"anies": [{"value": "17400.0", "module": "A1", "scenario": "Standard Scenario"}, {"value": "3220.0", "module": "A2", "scenario": "Standard Scenario"}, {"value": "9480.0", "module": "A3", "scenario": "Standard Scenario"}, {"value": "1910.0", "module": "A4", "scenario": "Norway Scenario"}, {"value": "684.0", "module": "A4", "scenario": "Sweden Scenario"}, {"value": "49.6", "module": "C1", "scenario": "Standard Scenario"}, {"value": "107.0", "module": "C2", "scenario": "Standard Scenario"}, {"value": "782.0", "module": "C3", "scenario": "Standard Scenario"}, {"value": "12.0", "module": "C4", "scenario": "Standard Scenario"}, {"value": "86.2", "module": "D", "scenario": "Standard Scenario"}, {"name": "referenceToUnitGroupDataSet", "value": {"shortDescription": [{"value": "MJ", "lang": "en"}], "type": "unit group data set", "refObjectId": "93a60a57-a3c8-11da-a746-0800200c9a66", "version": "03.00.000", "uri": "../unitgroups/93a60a57-a3c8-11da-a746-0800200c9a66.xml"}}]}}, {"referenceToLCIAMethodDataSet": {"shortDescription": [{"value": "Acidification potential, Accumulated Exceedance (AP)", "lang": "en"}, {"value": "Versauerungspotenzial, kumulierte Überschreitung (AP)", "lang": "de"}], "type": "LCIA method data set", "refObjectId": "b5c611c6-def3-11e6-bf01-fe55135034f3", "version": "01.03.010", "uri": "../lciamethods/b5c611c6-def3-11e6-bf01-fe55135034f3.xml"}, "meanAmount": 0.0, "other": {"anies": [{"value": "6.38", "module": "A1", "scenario": "Standard Scenario"}, {"value": "0.873", "module": "A2", "scenario": "Standard Scenario"}, {"value": "5.21", "module": "A3", "scenario": "Standard Scenario"}, {"value": "0.444", "module": "A4", "scenario": "Norway Scenario"}, {"value": "0.211", "module": "A4", "scenario": "Sweden Scenario"}, {"value": "0.0377", "module": "C1", "scenario": "Standard Scenario"}, {"value": "0.0411", "module": "C2", "scenario": "Standard Scenario"}, {"value": "0.579", "module": "C3", "scenario": "Standard Scenario"}, {"value": "0.00391", "module": "C4", "scenario": "Standard Scenario"}, {"value": "0.0329", "module": "D", "scenario": "Standard Scenario"}, {"name": "referenceToUnitGroupDataSet", "value": {"shortDescription": [{"value": "mol H+-eq.", "lang": "en"}], "type": "unit group data set", "refObjectId": "42e089ac-92bf-4bf2-8ca1-5fc40d18f2ed", "version": "00.01.000", "uri": "../unitgroups/42e089ac-92bf-4bf2-8ca1-5fc40d18f2ed.xml"}}]}}, {"referenceToLCIAMethodDataSet": {"shortDescription": [{"value": "Eutrophication potential - freshwater (EP-freshwater)", "lang": "en"}, {"value": "Eutrophierungspotenzial - Süßwasser (EP-freshwater)", "lang": "de"}], "type": "LCIA method data set", "refObjectId": "b53ec18f-7377-4ad3-86eb-cc3f4f276b2b", "version": "01.00.011", "uri": "../lciamethods/b53ec18f-7377-4ad3-86eb-cc3f4f276b2b.xml"}, "meanAmount": 0.0, "other": {"anies": [{"value": "0.0752", "module": "A1", "scenario": "Standard Scenario"}, {"value": "0.00168", "module": "A2", "scenario": "Standard Scenario"}, {"value": "0.0469", "module": "A3", "scenario": "Standard Scenario"}, {"value": "0.001", "module": "A4", "scenario": "Norway Scenario"}, {"value": "3.54E-4", "module": "A4", "scenario": "Sweden Scenario"}, {"value": "1.31E-5", "module": "C1", "scenario": "Standard Scenario"}, {"value": "7.15E-5", "module": "C2", "scenario": "Standard Scenario"}, {"value": "3.61E-4", "module": "C3", "scenario": "Standard Scenario"}, {"value": "5.78E-6", "module": "C4", "scenario": "Standard Scenario"}, {"value": "4.14E-4", "module": "D", "scenario": "Standard Scenario"}, {"name": "referenceToUnitGroupDataSet", "value": {"shortDescription": [{"value": "kg P-eq.", "lang": "en"}], "type": "unit group data set", "refObjectId": "0429039d-a61d-4590-ba67-aa4a20a810a1", "version": "30.00.000", "uri": "../unitgroups/0429039d-a61d-4590-ba67-aa4a20a810a1.xml"}}]}}, {"referenceToLCIAMethodDataSet": {"shortDescription": [{"value": "Eutrophication potential - marine (EP-marine)", "lang": "en"}, {"value": "Eutrophierungspotenzial - Salzwasser (EP-marine)", "lang": "de"}], "type": "LCIA method data set", "refObjectId": "b5c619fa-def3-11e6-bf01-fe55135034f3", "version": "02.00.011", "uri": "../lciamethods/b5c619fa-def3-11e6-bf01-fe55135034f3.xml"}, "meanAmount": 0.0, "other": {"anies": [{"value": "1.28", "module": "A1", "scenario": "Standard Scenario"}, {"value": "0.259", "module": "A2", "scenario": "Standard Scenario"}, {"value": "0.989", "module": "A3", "scenario": "Standard Scenario"}, {"value": "0.092", "module": "A4", "scenario": "Norway Scenario"}, {"value": "0.046", "module": "A4", "scenario": "Sweden Scenario"}, {"value": "0.0167", "module": "C1", "scenario": "Standard Scenario"}, {"value": "0.0145", "module": "C2", "scenario": "Standard Scenario"}, {"value": "0.253", "module": "C3", "scenario": "Standard Scenario"}, {"value": "0.00144", "module": "C4", "scenario": "Standard Scenario"}, {"value": "0.00405", "module": "D", "scenario": "Standard Scenario"}, {"name": "referenceToUnitGroupDataSet", "value": {"shortDescription": [{"value": "kg N-eq.", "lang": "en"}], "type": "unit group data set", "refObjectId": "d05bb823-ecdf-4686-8c40-bf1d9257859f", "version": "00.00.003", "uri": "../unitgroups/d05bb823-ecdf-4686-8c40-bf1d9257859f.xml"}}]}}, {"referenceToLCIAMethodDataSet": {"shortDescription": [{"value": "Eutrophication potential - terrestrial (EP-terrestrial)", "lang": "en"}, {"value": "Eutrophierungspotenzial - Land (EP-terrestrial)", "lang": "de"}], "type": "LCIA method data set", "refObjectId": "b5c614d2-def3-11e6-bf01-fe55135034f3", "version": "01.02.010", "uri": "../lciamethods/b5c614d2-def3-11e6-bf01-fe55135034f3.xml"}, "meanAmount": 0.0, "other": {"anies": [{"value": "14.1", "module": "A1", "scenario": "Standard Scenario"}, {"value": "2.86", "module": "A2", "scenario": "Standard Scenario"}, {"value": "12.1", "module": "A3", "scenario": "Standard Scenario"}, {"value": "1.03", "module": "A4", "scenario": "Norway Scenario"}, {"value": "0.513", "module": "A4", "scenario": "Sweden Scenario"}, {"value": "0.183", "module": "C1", "scenario": "Standard Scenario"}, {"value": "0.16", "module": "C2", "scenario": "Standard Scenario"}, {"value": "2.78", "module": "C3", "scenario": "Standard Scenario"}, {"value": "0.016", "module": "C4", "scenario": "Standard Scenario"}, {"value": "0.0209", "module": "D", "scenario": "Standard Scenario"}, {"name": "referenceToUnitGroupDataSet", "value": {"shortDescription": [{"value": "mol N-eq.", "lang": "en"}], "type": "unit group data set", "refObjectId": "71b4d617-0ec9-4d3f-b65e-e438940c2401", "version": "00.00.003", "uri": "../unitgroups/71b4d617-0ec9-4d3f-b65e-e438940c2401.xml"}}]}}, {"referenceToLCIAMethodDataSet": {"shortDescription": [{"value": "Potential Comparative Toxic Unit for ecosystems (ETP-fw)", "lang": "en"}, {"value": "Potenzielle Toxizitätsvergleichseinheit für Ökosysteme (ETP-fw)", "lang": "de"}], "type": "LCIA method data set", "refObjectId": "ee1082d1-b0f7-43ca-a1f0-21e2a4a74511", "version": "01.00.003", "uri": "../lciamethods/ee1082d1-b0f7-43ca-a1f0-21e2a4a74511.xml"}, "meanAmount": 0.0, "other": {"anies": [{"value": "40800.0", "module": "A1", "scenario": "Standard Scenario"}, {"value": "2580.0", "module": "A2", "scenario": "Standard Scenario"}, {"value": "74800.0", "module": "A3", "scenario": "Standard Scenario"}, {"value": "1530.0", "module": "A4", "scenario": "Norway Scenario"}, {"value": "545.0", "module": "A4", "scenario": "Sweden Scenario"}, {"value": "29.9", "module": "C1", "scenario": "Standard Scenario"}, {"value": "95.3", "module": "C2", "scenario": "Standard Scenario"}, {"value": "475.0", "module": "C3", "scenario": "Standard Scenario"}, {"value": "58.0", "module": "C4", "scenario": "Standard Scenario"}, {"value": "268.0", "module": "D", "scenario": "Standard Scenario"}, {"name": "referenceToUnitGroupDataSet", "value": {"shortDescription": [{"value": "CTUe", "lang": "en"}], "type": "unit group data set", "refObjectId": "aa959ded-f1eb-4efb-9c5c-2d60be36b3e6", "version": "00.00.003", "uri": "../unitgroups/aa959ded-f1eb-4efb-9c5c-2d60be36b3e6.xml"}}]}}, {"referenceToLCIAMethodDataSet": {"shortDescription": [{"value": "Global Warming Potential - biogenic (GWP-biogenic)", "lang": "en"}, {"value": "Globales Erwärmungspotenzial - biogen (GWP-biogenic)", "lang": "de"}], "type": "LCIA method data set", "refObjectId": "2356e1ab-0185-4db5-86e5-16de51c7485c", "version": "01.00.006", "uri": "../lciamethods/2356e1ab-0185-4db5-86e5-16de51c7485c.xml"}, "meanAmount": 0.0, "other": {"anies": [{"value": "5.32", "module": "A1", "scenario": "Standard Scenario"}, {"value": "0.114", "module": "A2", "scenario": "Standard Scenario"}, {"value": "16.8", "module": "A3", "scenario": "Standard Scenario"}, {"value": "0.0658", "module": "A4", "scenario": "Norway Scenario"}, {"value": "0.0223", "module": "A4", "scenario": "Sweden Scenario"}, {"value": "0.001", "module": "C1", "scenario": "Standard Scenario"}, {"value": "0.00327", "module": "C2", "scenario": "Standard Scenario"}, {"value": "0.0605", "module": "C3", "scenario": "Standard Scenario"}, {"value": "0.0207", "module": "C4", "scenario": "Standard Scenario"}, {"value": "-0.2", "module": "D", "scenario": "Standard Scenario"}, {"name": "referenceToUnitGroupDataSet", "value": {"shortDescription": [{"value": "kg CO2-eq.", "lang": "en"}], "type": "unit group data set", "refObjectId": "1ebf3012-d0db-4de2-aefd-ef30cedb0be1", "version": "30.00.000", "uri": "../unitgroups/1ebf3012-d0db-4de2-aefd-ef30cedb0be1.xml"}}]}}, {"referenceToLCIAMethodDataSet": {"shortDescription": [{"value": "Global Warming Potential - fossil fuels (GWP-fossil)", "lang": "en"}, {"value": "Globales Erwärmungspotenzial - fossil (GWP-fossil)", "lang": "de"}], "type": "LCIA method data set", "refObjectId": "5f635281-343e-44fb-83df-1971b155e6b6", "version": "01.00.009", "uri": "../lciamethods/5f635281-343e-44fb-83df-1971b155e6b6.xml"}, "meanAmount": 0.0, "other": {"anies": [{"value": "1270.0", "module": "A1", "scenario": "Standard Scenario"}, {"value": "213.0", "module": "A2", "scenario": "Standard Scenario"}, {"value": "656.0", "module": "A3", "scenario": "Standard Scenario"}, {"value": "127.0", "module": "A4", "scenario": "Norway Scenario"}, {"value": "45.6", "module": "A4", "scenario": "Sweden Scenario"}, {"value": "3.61", "module": "C1", "scenario": "Standard Scenario"}, {"value": "7.09", "module": "C2", "scenario": "Standard Scenario"}, {"value": "56.1", "module": "C3", "scenario": "Standard Scenario"}, {"value": "0.448", "module": "C4", "scenario": "Standard Scenario"}, {"value": "12.8", "module": "D", "scenario": "Standard Scenario"}, {"name": "referenceToUnitGroupDataSet", "value": {"shortDescription": [{"value": "kg CO2-eq.", "lang": "en"}], "type": "unit group data set", "refObjectId": "1ebf3012-d0db-4de2-aefd-ef30cedb0be1", "version": "30.00.000", "uri": "../unitgroups/1ebf3012-d0db-4de2-aefd-ef30cedb0be1.xml"}}]}}, {"referenceToLCIAMethodDataSet": {"shortDescription": [{"value": "Global Warming Potential - land use and land use change (GWP-luluc)", "lang": "en"}, {"value": "Globales Erwärmungspotenzial - luluc (GWP-luluc)", "lang": "de"}], "type": "LCIA method data set", "refObjectId": "4331bbdb-978a-490d-8707-eeb047f01a55", "version": "01.00.006", "uri": "../lciamethods/4331bbdb-978a-490d-8707-eeb047f01a55.xml"}, "meanAmount": 0.0, "other": {"anies": [{"value": "1.08", "module": "A1", "scenario": "Standard Scenario"}, {"value": "0.0747", "module": "A2", "scenario": "Standard Scenario"}, {"value": "1.35", "module": "A3", "scenario": "Standard Scenario"}, {"value": "0.046", "module": "A4", "scenario": "Norway Scenario"}, {"value": "0.0172", "module": "A4", "scenario": "Sweden Scenario"}, {"value": "2.84E-4", "module": "C1", "scenario": "Standard Scenario"}, {"value": "0.0026", "module": "C2", "scenario": "Standard Scenario"}, {"value": "0.00782", "module": "C3", "scenario": "Standard Scenario"}, {"value": "1.26E-4", "module": "C4", "scenario": "Standard Scenario"}, {"value": "-0.0168", "module": "D", "scenario": "Standard Scenario"}, {"name": "referenceToUnitGroupDataSet", "value": {"shortDescription": [{"value": "kg CO2-eq.", "lang": "en"}], "type": "unit group data set", "refObjectId": "1ebf3012-d0db-4de2-aefd-ef30cedb0be1", "version": "30.00.000", "uri": "../unitgroups/1ebf3012-d0db-4de2-aefd-ef30cedb0be1.xml"}}]}}, {"referenceToLCIAMethodDataSet": {"shortDescription": [{"value": "Global Warming Potential - total (GWP-total)", "lang": "en"}, {"value": "Globales Erwärmungspotenzial - total (GWP-total)", "lang": "de"}], "type": "LCIA method data set", "refObjectId": "6a37f984-a4b3-458a-a20a-64418c145fa2", "version": "04.00.017", "uri": "../lciamethods/6a37f984-a4b3-458a-a20a-64418c145fa2.xml"}, "meanAmount": 0.0, "other": {"anies": [{"value": "1280.0", "module": "A1", "scenario": "Standard Scenario"}, {"value": "214.0", "module": "A2", "scenario": "Standard Scenario"}, {"value": "674.0", "module": "A3", "scenario": "Standard Scenario"}, {"value": "127.0", "module": "A4", "scenario": "Norway Scenario"}, {"value": "45.7", "module": "A4", "scenario": "Sweden Scenario"}, {"value": "3.61", "module": "C1", "scenario": "Standard Scenario"}, {"value": "7.09", "module": "C2", "scenario": "Standard Scenario"}, {"value": "56.1", "module": "C3", "scenario": "Standard Scenario"}, {"value": "0.469", "module": "C4", "scenario": "Standard Scenario"}, {"value": "12.6", "module": "D", "scenario": "Standard Scenario"}, {"name": "referenceToUnitGroupDataSet", "value": {"shortDescription": [{"value": "kg CO2-eq.", "lang": "en"}], "type": "unit group data set", "refObjectId": "1ebf3012-d0db-4de2-aefd-ef30cedb0be1", "version": "30.00.000", "uri": "../unitgroups/1ebf3012-d0db-4de2-aefd-ef30cedb0be1.xml"}}]}}, {"referenceToLCIAMethodDataSet": {"shortDescription": [{"value": "Potential Comparative Toxic Unit for humans - cancer effects (HTP-c)", "lang": "en"}, {"value": "Potenzielle Toxizitätsvergleichseinheit für den Menschen - kanzerogene Wirkung (HTP-c)", "lang": "de"}], "type": "LCIA method data set", "refObjectId": "2299222a-bbd8-474f-9d4f-4dd1f18aea7c", "version": "01.00.004", "uri": "../lciamethods/2299222a-bbd8-474f-9d4f-4dd1f18aea7c.xml"}, "meanAmount": 0.0, "other": {"anies": [{"value": "1.24E-5", "module": "A1", "scenario": "Standard Scenario"}, {"value": "7.28E-8", "module": "A2", "scenario": "Standard Scenario"}, {"value": "3.39E-6", "module": "A3", "scenario": "Standard Scenario"}, {"value": "4.35E-8", "module": "A4", "scenario": "Norway Scenario"}, {"value": "1.61E-8", "module": "A4", "scenario": "Sweden Scenario"}, {"value": "1.05E-9", "module": "C1", "scenario": "Standard Scenario"}, {"value": "3.09E-9", "module": "C2", "scenario": "Standard Scenario"}, {"value": "1.66E-8", "module": "C3", "scenario": "Standard Scenario"}, {"value": "5.56E-10", "module": "C4", "scenario": "Standard Scenario"}, {"value": "-3.85E-10", "module": "D", "scenario": "Standard Scenario"}, {"name": "referenceToUnitGroupDataSet", "value": {"shortDescription": [{"value": "CTUh", "lang": "en"}], "type": "unit group data set", "refObjectId": "d4c9523e-2d7e-49fd-8469-998f547d3a70", "version": "00.00.003", "uri": "../unitgroups/d4c9523e-2d7e-49fd-8469-998f547d3a70.xml"}}]}}, {"referenceToLCIAMethodDataSet": {"shortDescription": [{"value": "Potential Comparative Toxic Unit for humans - non-cancer effects (HTP-nc)", "lang": "en"}, {"value": "Potenzielle Toxizitätsvergleichseinheit für den Menschen - nicht kanzerogene Wirkung (HTP-nc)", "lang": "de"}], "type": "LCIA method data set", "refObjectId": "3af763a5-b7a1-48c9-9cee-1f223481fcef", "version": "01.00.003", "uri": "../lciamethods/3af763a5-b7a1-48c9-9cee-1f223481fcef.xml"}, "meanAmount": 0.0, "other": {"anies": [{"value": "2.54E-4", "module": "A1", "scenario": "Standard Scenario"}, {"value": "2.81E-6", "module": "A2", "scenario": "Standard Scenario"}, {"value": "9.65E-5", "module": "A3", "scenario": "Standard Scenario"}, {"value": "1.61E-6", "module": "A4", "scenario": "Norway Scenario"}, {"value": "5.69E-7", "module": "A4", "scenario": "Sweden Scenario"}, {"value": "2.57E-8", "module": "C1", "scenario": "Standard Scenario"}, {"value": "1.04E-7", "module": "C2", "scenario": "Standard Scenario"}, {"value": "4.09E-7", "module": "C3", "scenario": "Standard Scenario"}, {"value": "4.54E-8", "module": "C4", "scenario": "Standard Scenario"}, {"value": "-2.69E-6", "module": "D", "scenario": "Standard Scenario"}, {"name": "referenceToUnitGroupDataSet", "value": {"shortDescription": [{"value": "CTUh", "lang": "en"}], "type": "unit group data set", "refObjectId": "d4c9523e-2d7e-49fd-8469-998f547d3a70", "version": "00.00.003", "uri": "../unitgroups/d4c9523e-2d7e-49fd-8469-998f547d3a70.xml"}}]}}, {"referenceToLCIAMethodDataSet": {"shortDescription": [{"value": "Potential Human exposure efficiency relative to U235 (IRP)", "lang": "en"}, {"value": "Potenzielle Wirkung durch Exposition des Menschen mit U235 (IRP)", "lang": "de"}], "type": "LCIA method data set", "refObjectId": "b5c632be-def3-11e6-bf01-fe55135034f3", "version": "01.00.012", "uri": "../lciamethods/b5c632be-def3-11e6-bf01-fe55135034f3.xml"}, "meanAmount": 0.0, "other": {"anies": [{"value": "67.4", "module": "A1", "scenario": "Standard Scenario"}, {"value": "14.1", "module": "A2", "scenario": "Standard Scenario"}, {"value": "50.7", "module": "A3", "scenario": "Standard Scenario"}, {"value": "8.34", "module": "A4", "scenario": "Norway Scenario"}, {"value": "2.99", "module": "A4", "scenario": "Sweden Scenario"}, {"value": "0.213", "module": "C1", "scenario": "Standard Scenario"}, {"value": "0.448", "module": "C2", "scenario": "Standard Scenario"}, {"value": "3.48", "module": "C3", "scenario": "Standard Scenario"}, {"value": "0.0599", "module": "C4", "scenario": "Standard Scenario"}, {"value": "-0.263", "module": "D", "scenario": "Standard Scenario"}, {"name": "referenceToUnitGroupDataSet", "value": {"shortDescription": [{"value": "kgBq U235-eq.", "lang": "en"}], "type": "unit group data set", "refObjectId": "456b05bf-1415-44a9-9993-02452f554c09", "version": "00.00.003", "uri": "../unitgroups/456b05bf-1415-44a9-9993-02452f554c09.xml"}}]}}, {"referenceToLCIAMethodDataSet": {"shortDescription": [{"value": "Depletion potential of the stratospheric ozone layer (ODP)", "lang": "en"}, {"value": "Abbaupotenzial der stratosphärischen Ozonschicht (ODP)", "lang": "de"}], "type": "LCIA method data set", "refObjectId": "b5c629d6-def3-11e6-bf01-fe55135034f3", "version": "02.00.013", "uri": "../lciamethods/b5c629d6-def3-11e6-bf01-fe55135034f3.xml"}, "meanAmount": 0.0, "other": {"anies": [{"value": "1.02E-4", "module": "A1", "scenario": "Standard Scenario"}, {"value": "4.85E-5", "module": "A2", "scenario": "Standard Scenario"}, {"value": "7.63E-5", "module": "A3", "scenario": "Standard Scenario"}, {"value": "2.87E-5", "module": "A4", "scenario": "Norway Scenario"}, {"value": "1.03E-5", "module": "A4", "scenario": "Sweden Scenario"}, {"value": "7.79E-7", "module": "C1", "scenario": "Standard Scenario"}, {"value": "1.56E-6", "module": "C2", "scenario": "Standard Scenario"}, {"value": "1.19E-5", "module": "C3", "scenario": "Standard Scenario"}, {"value": "1.61E-7", "module": "C4", "scenario": "Standard Scenario"}, {"value": "1.52E-7", "module": "D", "scenario": "Standard Scenario"}, {"name": "referenceToUnitGroupDataSet", "value": {"shortDescription": [{"value": "kg CFC-11-eq.", "lang": "en"}], "type": "unit group data set", "refObjectId": "d9e957c9-7309-4474-bf3a-7777df6c4e5b", "version": "25.00.000", "uri": "../unitgroups/d9e957c9-7309-4474-bf3a-7777df6c4e5b.xml"}}]}}, {"referenceToLCIAMethodDataSet": {"shortDescription": [{"value": "Potential incidence of disease due to PM emissions (PM)", "lang": "en"}, {"value": "Potenzielles Auftreten von Krankheiten aufgrund von Feinstaubemissionen (PM)", "lang": "de"}], "type": "LCIA method data set", "refObjectId": "b5c602c6-def3-11e6-bf01-fe55135034f3", "version": "02.00.012", "uri": "../lciamethods/b5c602c6-def3-11e6-bf01-fe55135034f3.xml"}, "meanAmount": 0.0, "other": {"anies": [{"value": "1.14E-4", "module": "A1", "scenario": "Standard Scenario"}, {"value": "1.49E-5", "module": "A2", "scenario": "Standard Scenario"}, {"value": "3.87E-5", "module": "A3", "scenario": "Standard Scenario"}, {"value": "7.97E-6", "module": "A4", "scenario": "Norway Scenario"}, {"value": "2.82E-6", "module": "A4", "scenario": "Sweden Scenario"}, {"value": "1.0E-6", "module": "C1", "scenario": "Standard Scenario"}, {"value": "6.37E-7", "module": "C2", "scenario": "Standard Scenario"}, {"value": "1.51E-5", "module": "C3", "scenario": "Standard Scenario"}, {"value": "8.05E-8", "module": "C4", "scenario": "Standard Scenario"}, {"value": "5.17E-7", "module": "D", "scenario": "Standard Scenario"}, {"name": "referenceToUnitGroupDataSet", "value": {"shortDescription": [{"value": "Disease incidence", "lang": "en"}], "type": "unit group data set", "refObjectId": "3883559b-648f-4afc-8ba2-0bd24f3affa3", "version": "00.00.003", "uri": "../unitgroups/3883559b-648f-4afc-8ba2-0bd24f3affa3.xml"}}]}}, {"referenceToLCIAMethodDataSet": {"shortDescription": [{"value": "Photochemical Ozone Creation Potential (POCP)", "lang": "en"}, {"value": "Bildungspotenzial für troposphärisches Ozon (POCP)", "lang": "de"}], "type": "LCIA method data set", "refObjectId": "b5c610fe-def3-11e6-bf01-fe55135034f3", "version": "02.00.015", "uri": "../lciamethods/b5c610fe-def3-11e6-bf01-fe55135034f3.xml"}, "meanAmount": 0.0, "other": {"anies": [{"value": "5.74", "module": "A1", "scenario": "Standard Scenario"}, {"value": "0.877", "module": "A2", "scenario": "Standard Scenario"}, {"value": "3.04", "module": "A3", "scenario": "Standard Scenario"}, {"value": "0.364", "module": "A4", "scenario": "Norway Scenario"}, {"value": "0.167", "module": "A4", "scenario": "Sweden Scenario"}, {"value": "0.0502", "module": "C1", "scenario": "Standard Scenario"}, {"value": "0.0456", "module": "C2", "scenario": "Standard Scenario"}, {"value": "0.763", "module": "C3", "scenario": "Standard Scenario"}, {"value": "0.00457", "module": "C4", "scenario": "Standard Scenario"}, {"value": "0.0604", "module": "D", "scenario": "Standard Scenario"}, {"name": "referenceToUnitGroupDataSet", "value": {"shortDescription": [{"value": "kg NMVOC-eq.", "lang": "en"}], "type": "unit group data set", "refObjectId": "d27c25f8-fbc1-44c6-b47b-4adbae4199c6", "version": "00.00.003", "uri": "../unitgroups/d27c25f8-fbc1-44c6-b47b-4adbae4199c6.xml"}}]}}, {"referenceToLCIAMethodDataSet": {"shortDescription": [{"value": "Potential Soil quality index (SQP)", "lang": "en"}, {"value": "Potenzieller Bodenqualitätsindex (SQP)", "lang": "de"}], "type": "LCIA method data set", "refObjectId": "b2ad6890-c78d-11e6-9d9d-cec0c932ce01", "version": "01.00.011", "uri": "../lciamethods/b2ad6890-c78d-11e6-9d9d-cec0c932ce01.xml"}, "meanAmount": 0.0, "other": {"anies": [{"value": "5330.0", "module": "A1", "scenario": "Standard Scenario"}, {"value": "2220.0", "module": "A2", "scenario": "Standard Scenario"}, {"value": "8610.0", "module": "A3", "scenario": "Standard Scenario"}, {"value": "1310.0", "module": "A4", "scenario": "Norway Scenario"}, {"value": "459.0", "module": "A4", "scenario": "Sweden Scenario"}, {"value": "6.33", "module": "C1", "scenario": "Standard Scenario"}, {"value": "92.7", "module": "C2", "scenario": "Standard Scenario"}, {"value": "118.0", "module": "C3", "scenario": "Standard Scenario"}, {"value": "29.4", "module": "C4", "scenario": "Standard Scenario"}, {"value": "-731.0", "module": "D", "scenario": "Standard Scenario"}, {"name": "referenceToUnitGroupDataSet", "value": {"shortDescription": [{"value": "dimensionless", "lang": "en"}], "type": "unit group data set", "refObjectId": "f130951c-e67f-4f7f-8dd4-665de3974e18", "version": "00.00.004", "uri": "../unitgroups/f130951c-e67f-4f7f-8dd4-665de3974e18.xml"}}]}}, {"referenceToLCIAMethodDataSet": {"shortDescription": [{"value": "Water (user) deprivation potential (WDP)", "lang": "en"}, {"value": "Wasser-Entzugspotenzial (Benutzer) (WDP)", "lang": "de"}], "type": "LCIA method data set", "refObjectId": "b2ad66ce-c78d-11e6-9d9d-cec0c932ce01", "version": "03.00.015", "uri": "../lciamethods/b2ad66ce-c78d-11e6-9d9d-cec0c932ce01.xml"}, "meanAmount": 0.0, "other": {"anies": [{"value": "720.0", "module": "A1", "scenario": "Standard Scenario"}, {"value": "8.97", "module": "A2", "scenario": "Standard Scenario"}, {"value": "420.0", "module": "A3", "scenario": "Standard Scenario"}, {"value": "5.35", "module": "A4", "scenario": "Norway Scenario"}, {"value": "1.89", "module": "A4", "scenario": "Sweden Scenario"}, {"value": "0.0665", "module": "C1", "scenario": "Standard Scenario"}, {"value": "0.382", "module": "C2", "scenario": "Standard Scenario"}, {"value": "1.36", "module": "C3", "scenario": "Standard Scenario"}, {"value": "0.0566", "module": "C4", "scenario": "Standard Scenario"}, {"value": "2.5", "module": "D", "scenario": "Standard Scenario"}, {"name": "referenceToUnitGroupDataSet", "value": {"shortDescription": [{"value": "m3 world eq. deprived", "lang": "en"}], "type": "unit group data set", "refObjectId": "6ae2df01-888e-46c8-b17d-49fa3869b476", "version": "00.00.003", "uri": "../unitgroups/6ae2df01-888e-46c8-b17d-49fa3869b476.xml"}}]}}]}, "otherAttributes": {"{http://www.indata.network/EPD/2019}epd-version": "1.2"}, "version": "1.1"}