{"processInformation": {"dataSetInformation": {"UUID": "b922ae45-0960-4d94-b2a0-ae6f7fcc11b4", "name": {"baseName": [{"value": "Grobblech (Salzgitter AG)", "lang": "de"}, {"value": "Heavy Plate (Salzgitter AG)", "lang": "en"}], "functionalUnitFlowProperties": [{"lang": "de"}]}, "classificationInformation": {"classification": [{"class": [{"value": "Metalle", "level": 0, "classId": "4"}, {"value": "Stahl und Eisen", "level": 1, "classId": "4.1"}, {"value": "Stahlbleche", "level": 2, "classId": "4.1.04"}], "name": "OEKOBAU.DAT"}, {"class": [{"value": "02 Bauprodukte", "level": 0}, {"value": "Metallbauprodukte und Zubehör", "level": 1}, {"value": "Baustähle", "level": 2}], "name": "IBUCategories"}]}, "generalComment": [{"value": "Die vorliegende EPD bezieht sich auf alle Produkte der Ilsenburger Grobblech inklusive der Grobbleche der Marken BRINAR®, MAXIL® und RESTIL® sowie die Produkte der Salzgitter Mannesmann Grobblech.\n\nFür das Inverkehrbringen des Produkts in der EU/EFTA (mit Ausnahme der Schweiz) gilt die Verordnung (EU) Nr. 305/2011 (CPR). Das Produkt benötigt eine Leistungserklärung unter Berücksichtigung der EN 10025 (Warmgewalzte Erzeugnisse aus Baustählen) und die CE-Kennzeichnung. \n\nFür die Verwendung gelten die jeweiligen nationalen Bestimmungen.", "lang": "de"}, {"value": "This EPD relates to all products of Ilsenburger Grobblech, including the heavy plates of the BRINAR®, MAXIL® and RESTIL® brands as well as the products of Salzgitter Mannesmann Grobblech. (EU) Directive No. 305/2011 (CPR) applies for placing the product on the market in the EU/EFTA (with the exception of Switzerland). The product requires a declaration of performance taking into account EN 10025 (Hot rolled products of structural steels) and CE marking.\n\nThe respective national regulations apply for usage.", "lang": "en"}]}, "quantitativeReference": {"referenceToReferenceFlow": [0]}, "time": {"referenceYear": 2022, "dataSetValidUntil": 2027, "other": {"anies": [{"name": "publicationDateOfEPD", "value": 1644537600000}]}}, "geography": {"locationOfOperationSupplyOrProduction": {"location": "DE"}}, "technology": {"technologyDescriptionAndIncludedProcesses": [{"value": "Das Vormaterial für Grobbleche aus den Walzwerken der Ilsenburger Grobblech und der Salzgitter Mannesmann Grobblech sind Brammen, die über die Primärroute (Hochofen mit Konverter) erzeugt werden. Die Brammen werden in Wärmeöfen der Walzwerke erneut auf Temperaturen zwischen 1.000°C und 1.250 °C erwärmt und in einem reversierenden Walzverfahren zu Grobblechen in der individuell durch den Kunden definierten Länge und Breite ausgewalzt. Die Walzgerüste der Ilsenburger Grobblech und der Salzgitter Mannesmann Grobblech sind sogenannte Quartowalzgerüste, bestehend aus vier Walzen: zwei Arbeitswalzen und zwei Stützwalzen. \nTechnische Daten: \nDie vorliegende EPD umfasst alle Produkte der Ilsenburger Grobblech und der Salzgitter Mannesmann Grobblech in diversen Stahlgüten, Abmessungen, Formen und Auslieferungszuständen. Zudem inkludiert sie Grobbleche der Marken BRINAR®, MAXIL® und RESTIL® der Ilsenburger Grobblech. \n\nDie gütenspezifischen Informationen zu Toleranzangaben können in den für den Anwendungsbereich definierten Normen, zum Beispiel EN 10029 und EN 10025, eingesehen werden. \n\nWeiterhin gelten die jeweiligen Angaben in der Leistungserklärung. \nDeklarierte Einheit: \nAls Repräsentant der Produktgruppe Grobbech, dient 1 t Grobblech als deklarierte Einheit.", "lang": "de"}, {"value": "The starting material for heavy plate from the rolling mills of Ilsenburger Grobblech and Salzgitter Mannesmann Grobblech are slabs produced via the primary route (blast furnace with converter). The slabs are reheated in the rolling mills’ heating furnaces to temperatures between 1,000 °C and 1,250 °C and rolled out in a reversing rolling process to produce heavy plate in the lengths and widths individually defined by the customer. The rolling stands of Ilsenburger Grobblech and Salzgitter Mannesmann Grobblech are so-called quarto rolling stands, consisting of four rolls: two work rolls and two back-up rolls. \nTechnical data: \nThis EPD covers all products of Ilsenburger Grobblech and Salzgitter Mannesmann Grobblech in various steel grades, dimensions, shapes and delivery states. It also includes heavy plates of the brands BRINAR®, MAXIL® and RESTIL® of Ilsenburger Grobblech. \n\n\nThe quality-specific information on tolerance specifications can be found in the standards defined for the area of application, for example EN 10029 and EN 10025. \n\nFurthermore, the respective information in the Declaration of Performance applies. \nDeclared unit: \nAs a representative of the heavy plate product group, one tonne heavy plate serves as the declared unit.", "lang": "en"}], "technologicalApplicability": [{"value": "Die Einsatzgebiete für Grobbleche der Ilsenburger Grobblech und der Salzgitter Mannesmann Grobblech liegen unter anderem in folgenden Bereichen:\n\n\nStahl- und Brückenbau\nTank- und Anlagenbau\nWindindustrie (On- und Offshore-Konstruktionen)\nKessel- und Apparatebau\nYellow Goods (hoch- und verschleißfeste Stähle für den Fahrzeug- und Kranbau)\nMaschinen- und Metallbau\nSchiffbau\nRohrleitungen", "lang": "de"}, {"value": "The areas of application for heavy plate from Ilsenburger Grobblech and Salzgitter Mannesmann Grobblech include the following:\n\n\nSteel and bridge construction\nTank and plant construction\nWind industry (onshore and offshore constructions)\nBoiler and pressure vessel engineering\nYellow Goods (high-strength and wear-resistant steels for vehicle and crane construction)\nMechanical engineering and metal construction\nShipbuilding\nPipelines", "lang": "en"}]}}, "modellingAndValidation": {"LCIMethodAndAllocation": {"typeOfDataSet": "EPD", "referenceToLCAMethodDetails": [{"shortDescription": [{"value": "Baustähle.pdf", "lang": "de"}], "type": "source data set", "refObjectId": "1dcfe8ce-f293-42b6-b217-e335f198b5cf"}], "other": {"anies": [{"name": "subType", "value": "specific dataset"}]}}, "dataSourcesTreatmentAndRepresentativeness": {"referenceToDataSource": [{"shortDescription": [{"value": "GaBi Database (all versions)", "lang": "de"}], "type": "source data set", "refObjectId": "28d74cc0-db8b-4d7e-bc44-5f6d56ce0c4a"}, {"shortDescription": [{"value": "GaBi Database Edition 2021, CUP 2021.02", "lang": "de"}], "type": "source data set", "refObjectId": "90321ffe-9ebb-4946-886c-338efe6fbf26"}], "useAdviceForDataSet": [{"value": "Gültigkeitsbereich: \nDiese Umwelt Produktdeklaration ist gültig für Grobblech aus den Walzwerken der Ilsenburger Grobblech in Ilsenburg und der Salzgitter Mannesmann Grobblech in Mülheim an der Ruhr. Sie behandelt thermomechanisch gewalzte, wärmebehandelte, normal- und hochfeste Grobbleche beider Werke. Die Grobblechprodukte werden aus Brammen hergestellt, die aus einer primären Stahlherstellungsroute stammen (Hochofenroute). Die EPD wurde nach den Vorgaben der EN 15804+A2 erstellt. Im Folgenden wird die Norm vereinfacht als EN 15804 bezeichnet. \nSystemgrenze: \nTyp der EPD: Von der Wiege bis zum Werkstor mit den Modulen C1–C4 und Modul D. \n\n Die EPD umfasst folgende Lebenszyklusphasen:\n\nA1: Hochofenbasierte Stahlherstellung auf Basis von Eisenerz\nA2: Transport der Brammen zu den Grobblechproduzenten\nA3: Grobblechherstellung\nC3-C4: Entsorgungsstadium\nD: Gutschriften und Lasten außerhalb der Systemgrenze\n\nIn allen Modulen werden zusätzlich zu den direkten Verbräuchen auch die Aufwände zur Herstellung der Rohstoffe, der Hilfsstoffe, der Energieträger sowie die Abwasser- und Reststoffentsorgung betrachtet.  \n\nFür die Module C3-C4 wird angenommen, dass keine weiteren stofflichen und energetischen Aufwände für die Abfallbehandlung bestehen und kein Material beseitigt werden muss.\n\nIn Modul D werden das Wiederverwendungs- und Recyclingpotenzial berücksichtigt. Die Gutschrift des Recyclinganteils erfolgt nach dem Ansatz der „theoretischen 100 % primären Hochofenroute“ entsprechend Worldsteel 2017.", "lang": "de"}, {"value": "Scope: \nThis Environmental Product Declaration applies for heavy plate from the rolling mills at Ilsenburger Grobblech in Ilsenburg and Salzgitter Mannesmann Grobblech in Mülheim an der Ruhr. It concerns thermomechanically-rolled, heat-treated, normalized and high-strength heavy plates from both mills. The heavy plate products are made from slabs that come from a primary steel-making route (blast furnace route). This EPD was drawn up in accordance with the specifications of the EN 15804+A2. This standard is referred to as EN 15804 hereinafter. \nSystem boundary: \nType of EPD: cradle to gate with Modules C1–C4 and Module D. \n\n\nThe EPD comprises the following life cycle phases: \n\nA1: Blast furnace-based steel production on the basis of iron ore\nA2: Transport of the slabs to the heavy plate producers\nA3: Heavy plate production\nC3-C4: End-of-life stage\nD: Benefits and loads beyond the system boundaries \n\nIn all modules, in addition to direct consumption, the costs for the production of raw materials, auxiliary materials, energy sources and wastewater and residue disposal are also considered. \n\n\nIt is assumed for Modules C3-C4 that there are no other material or energetic expenses for waste processing and that no materials need to be disposed of. \n\n\nModule D takes consideration of the re-use and recycling potential. Recycling credits are allocated in line with the “theoretically 100% primary furnace route” approach, in accordance with Worldsteel 2017.", "lang": "en"}], "other": {"anies": [{"name": "referenceToOriginalEPD", "value": {"shortDescription": {"value": "Grobblech.pdf", "defaultValue": "Grobblech.pdf", "lstrings": [{"lang": "de", "value": "Grobblech.pdf"}]}, "type": "source data set", "uuid": {"uuid": "c3346044-bd2a-46b5-9c51-7d68ce0f31a2"}, "refObjectId": "c3346044-bd2a-46b5-9c51-7d68ce0f31a2", "resourceURLs": ["https://oekobaudat.de/OEKOBAU.DAT/resource/sources/c3346044-bd2a-46b5-9c51-7d68ce0f31a2/Grobblech_15693.pdf?version=00.01.000"]}}]}}, "validation": {"review": [{"referenceToNameOfReviewerAndInstitution": [{"shortDescription": [{"value": "Institut Bauen und Umwelt e. V.", "lang": "de"}], "type": "contact data set", "refObjectId": "d111dbec-b024-4be5-86c5-752d6eb2cf95", "uri": "../contacts/d111dbec-b024-4be5-86c5-752d6eb2cf95.xml"}], "type": "Accredited third party review"}]}, "complianceDeclarations": {"compliance": [{"referenceToComplianceSystem": {"shortDescription": [{"value": "DIN EN 15804+A2", "lang": "de"}], "type": "source data set", "refObjectId": "c0016b33-8cf7-415c-ac6e-deba0d21440d", "uri": "../sources/c0016b33-8cf7-415c-ac6e-deba0d21440d.xml"}}, {"referenceToComplianceSystem": {"shortDescription": [{"value": "ISO 14025", "lang": "de"}], "type": "source data set", "refObjectId": "4f2eb655-6e44-4874-a95a-e28f5442cd4d", "uri": "../sources/4f2eb655-6e44-4874-a95a-e28f5442cd4d.xml"}}]}}, "administrativeInformation": {"commissionerAndGoal": {"referenceToCommissioner": [{"shortDescription": [{"value": "Salzgitter AG", "lang": "de"}], "type": "contact data set", "refObjectId": "6333d1b0-b652-4178-bfa4-1ae7c2274f0f", "uri": "../contacts/6333d1b0-b652-4178-bfa4-1ae7c2274f0f.xml"}]}, "dataGenerator": {"referenceToPersonOrEntityGeneratingTheDataSet": [{"shortDescription": [{"value": "Salzgitter Mannesmann Forschung GmbH", "lang": "de"}], "type": "contact data set", "refObjectId": "5efd859f-8574-4295-86e8-9d78a497a753", "uri": "../contacts/5efd859f-8574-4295-86e8-9d78a497a753.xml"}]}, "dataEntryBy": {"timeStamp": 1644585758278, "referenceToDataSetFormat": [{"shortDescription": [{"value": "ILCD Format", "lang": "de"}], "type": "source data set", "refObjectId": "a97a0155-0234-4b87-b4ce-a45da52f2a40", "uri": "../sources/a97a0155-0234-4b87-b4ce-a45da52f2a40.xml"}, {"shortDescription": [{"value": "EPD-Datenformaterweiterungen v1.2", "lang": "de"}, {"value": "EPD Data Format Extensions v1.2", "lang": "en"}], "type": "source data set", "refObjectId": "a29449fd-aa2f-4de8-b5d7-4b06b43c6fde", "uri": "../sources/a29449fd-aa2f-4de8-b5d7-4b06b43c6fde.xml"}]}, "publicationAndOwnership": {"dataSetVersion": "00.03.000", "dateOfLastRevision": 1644572520000, "referenceToRegistrationAuthority": {"shortDescription": [{"value": "Institut Bauen und Umwelt e. V.", "lang": "de"}], "type": "contact data set", "refObjectId": "d111dbec-b024-4be5-86c5-752d6eb2cf95", "uri": "../contacts/d111dbec-b024-4be5-86c5-752d6eb2cf95.xml"}, "registrationNumber": "EPD-SMM-20210289-IBB1-DE", "referenceToOwnershipOfDataSet": {"shortDescription": [{"value": "Salzgitter AG", "lang": "de"}], "type": "contact data set", "refObjectId": "6333d1b0-b652-4178-bfa4-1ae7c2274f0f", "uri": "../contacts/6333d1b0-b652-4178-bfa4-1ae7c2274f0f.xml"}, "copyright": true, "licenseType": "Free of charge for all users and uses", "accessRestrictions": [{"value": "None", "lang": "en"}], "other": {"anies": [{"name": "referenceToPublisher", "value": {"shortDescription": [{"value": "Institut Bauen und Umwelt e. V.", "lang": "de"}], "type": "contact data set", "refObjectId": "d111dbec-b024-4be5-86c5-752d6eb2cf95", "uri": "../contacts/d111dbec-b024-4be5-86c5-752d6eb2cf95.xml"}}]}}}, "exchanges": {"exchange": [{"dataSetInternalID": 0, "referenceToFlowDataSet": {"shortDescription": [{"value": "Grobblech (Grobblech)", "lang": "de"}], "type": "flow data set", "refObjectId": "b4e76770-8de6-aead-ef48-2759a499bfce", "uri": "../flows/b4e76770-8de6-aead-ef48-2759a499bfce.xml"}, "meanAmount": 1.0, "referencesToDataSource": {}, "referenceFlow": true, "resolvedFlowVersion": "00.03.000", "resultingflowAmount": 1000.0, "flowProperties": [{"name": [{"lang": "de", "value": "biogener Kohlenstoffgehalt"}, {"lang": "en", "value": "Carbon content (biogenic)"}], "uuid": "62e503ce-544a-4599-b2ad-bcea15a7bf20", "meanValue": 0.0}, {"name": [{"lang": "en", "value": "Mass"}, {"lang": "de", "value": "Masse"}], "uuid": "93a60a56-a3c8-11da-a746-0800200b9a66", "referenceFlowProperty": true, "meanValue": 1000.0, "referenceUnit": "kg", "unitGroupUUID": "ad38d542-3fe9-439d-9b95-2f5f7752acaf"}, {"name": [{"lang": "de", "value": "Masse"}, {"lang": "en", "value": "Mass"}], "uuid": "93a60a56-a3c8-11da-a746-0800200b9a66", "referenceFlowProperty": true, "meanValue": 7850.0}], "materialProperties": [{"name": "gross density", "value": "7850.0", "unit": "kg/m^3", "unitDescription": "kilograms per cubic metre"}], "typeOfFlow": "Product flow", "classification": {"classHierarchy": "Metalle / Stahl und Eisen / Stahlbleche", "name": "OEKOBAU.DAT"}}, {"dataSetInternalID": 1, "referenceToFlowDataSet": {"shortDescription": [{"value": "Erneuerbare Primärenergie als Energieträger (PERE)", "lang": "de"}, {"value": "Renewable primary energy as energy carrier (PERE)", "lang": "en"}], "type": "flow data set", "refObjectId": "20f32be5-0398-4288-9b6d-accddd195317", "uri": "../flows/20f32be5-0398-4288-9b6d-accddd195317.xml"}, "exchange direction": "INPUT", "other": {"anies": [{"name": "referenceToUnitGroupDataSet", "value": {"shortDescription": [{"value": "MJ", "lang": "de"}], "type": "unit group data set", "refObjectId": "93a60a57-a3c8-11da-a746-0800200c9a66", "uri": "../unitgroups/93a60a57-a3c8-11da-a746-0800200c9a66.xml"}}, {"value": "1280", "module": "A1-A3"}, {"value": "0", "module": "C3"}, {"value": "0", "module": "C4"}, {"value": "1490", "module": "D"}]}, "resolvedFlowVersion": "38.00.000", "flowProperties": [], "typeOfFlow": "Other flow", "classification": {"classHierarchy": "Quantities", "name": "GaBiCategories"}}, {"dataSetInternalID": 2, "referenceToFlowDataSet": {"shortDescription": [{"value": "Erneuerbare Primärenergie zur stofflichen Nutzung (PERM)", "lang": "de"}, {"value": "Renewable primary energy resources as material utilization (PERM)", "lang": "en"}], "type": "flow data set", "refObjectId": "fb3ec0de-548d-4508-aea5-00b73bf6f702", "uri": "../flows/fb3ec0de-548d-4508-aea5-00b73bf6f702.xml"}, "exchange direction": "INPUT", "other": {"anies": [{"name": "referenceToUnitGroupDataSet", "value": {"shortDescription": [{"value": "MJ", "lang": "de"}], "type": "unit group data set", "refObjectId": "93a60a57-a3c8-11da-a746-0800200c9a66", "uri": "../unitgroups/93a60a57-a3c8-11da-a746-0800200c9a66.xml"}}, {"value": "0", "module": "A1-A3"}, {"value": "0", "module": "C3"}, {"value": "0", "module": "C4"}, {"value": "0", "module": "D"}]}, "resolvedFlowVersion": "38.00.000", "flowProperties": [], "typeOfFlow": "Other flow", "classification": {"classHierarchy": "Quantities", "name": "GaBiCategories"}}, {"dataSetInternalID": 3, "referenceToFlowDataSet": {"shortDescription": [{"value": "Total erneuerbare Primärenergie (PERT)", "lang": "de"}, {"value": "Total use of renewable primary energy resources (PERT)", "lang": "en"}], "type": "flow data set", "refObjectId": "53f97275-fa8a-4cdd-9024-65936002acd0", "uri": "../flows/53f97275-fa8a-4cdd-9024-65936002acd0.xml"}, "exchange direction": "INPUT", "other": {"anies": [{"name": "referenceToUnitGroupDataSet", "value": {"shortDescription": [{"value": "MJ", "lang": "de"}], "type": "unit group data set", "refObjectId": "93a60a57-a3c8-11da-a746-0800200c9a66", "uri": "../unitgroups/93a60a57-a3c8-11da-a746-0800200c9a66.xml"}}, {"value": "1280", "module": "A1-A3"}, {"value": "0", "module": "C3"}, {"value": "0", "module": "C4"}, {"value": "1490", "module": "D"}]}, "resolvedFlowVersion": "38.00.000", "flowProperties": [], "typeOfFlow": "Other flow", "classification": {"classHierarchy": "Quantities / Environmental quantities / EPD EN 15804 / LCI indicators", "name": "GaBiCategories"}}, {"dataSetInternalID": 4, "referenceToFlowDataSet": {"shortDescription": [{"value": "Nicht-erneuerbare Primärenergie als Energieträger (PENRE)", "lang": "de"}, {"value": "Non renewable primary energy as energy carrier (PENRE)", "lang": "en"}], "type": "flow data set", "refObjectId": "ac857178-2b45-46ec-892a-a9a4332f0372", "uri": "../flows/ac857178-2b45-46ec-892a-a9a4332f0372.xml"}, "exchange direction": "INPUT", "other": {"anies": [{"name": "referenceToUnitGroupDataSet", "value": {"shortDescription": [{"value": "MJ", "lang": "de"}], "type": "unit group data set", "refObjectId": "93a60a57-a3c8-11da-a746-0800200c9a66", "uri": "../unitgroups/93a60a57-a3c8-11da-a746-0800200c9a66.xml"}}, {"value": "22100", "module": "A1-A3"}, {"value": "0", "module": "C3"}, {"value": "0", "module": "C4"}, {"value": "-12700", "module": "D"}]}, "resolvedFlowVersion": "38.00.000", "flowProperties": [], "typeOfFlow": "Other flow", "classification": {"classHierarchy": "Quantities", "name": "GaBiCategories"}}, {"dataSetInternalID": 5, "referenceToFlowDataSet": {"shortDescription": [{"value": "Nicht-erneuerbare Primärenergie zur stofflichen Nutzung (PENRM)", "lang": "de"}, {"value": "Non renewable primary energy as material utilization (PENRM)", "lang": "en"}], "type": "flow data set", "refObjectId": "1421caa0-679d-4bf4-b282-0eb850ccae27", "uri": "../flows/1421caa0-679d-4bf4-b282-0eb850ccae27.xml"}, "exchange direction": "INPUT", "other": {"anies": [{"name": "referenceToUnitGroupDataSet", "value": {"shortDescription": [{"value": "MJ", "lang": "de"}], "type": "unit group data set", "refObjectId": "93a60a57-a3c8-11da-a746-0800200c9a66", "uri": "../unitgroups/93a60a57-a3c8-11da-a746-0800200c9a66.xml"}}, {"value": "0", "module": "A1-A3"}, {"value": "0", "module": "C3"}, {"value": "0", "module": "C4"}, {"value": "0", "module": "D"}]}, "resolvedFlowVersion": "38.00.000", "flowProperties": [], "typeOfFlow": "Other flow", "classification": {"classHierarchy": "Quantities", "name": "GaBiCategories"}}, {"dataSetInternalID": 6, "referenceToFlowDataSet": {"shortDescription": [{"value": "Total nicht erneuerbare Primärenergie (PENRT)", "lang": "de"}, {"value": "Total use of non renewable primary energy resources (PENRT)", "lang": "en"}], "type": "flow data set", "refObjectId": "06159210-646b-4c8d-8583-da9b3b95a6c1", "uri": "../flows/06159210-646b-4c8d-8583-da9b3b95a6c1.xml"}, "exchange direction": "INPUT", "other": {"anies": [{"name": "referenceToUnitGroupDataSet", "value": {"shortDescription": [{"value": "MJ", "lang": "de"}], "type": "unit group data set", "refObjectId": "93a60a57-a3c8-11da-a746-0800200c9a66", "uri": "../unitgroups/93a60a57-a3c8-11da-a746-0800200c9a66.xml"}}, {"value": "22100", "module": "A1-A3"}, {"value": "0", "module": "C3"}, {"value": "0", "module": "C4"}, {"value": "-12700", "module": "D"}]}, "resolvedFlowVersion": "38.00.000", "flowProperties": [], "typeOfFlow": "Other flow", "classification": {"classHierarchy": "Quantities / Environmental quantities / EPD EN 15804 / LCI indicators", "name": "GaBiCategories"}}, {"dataSetInternalID": 7, "referenceToFlowDataSet": {"shortDescription": [{"value": "Einsatz von Sekundärstoffen (SM)", "lang": "de"}, {"value": "Use of secondary material (SM)", "lang": "en"}], "type": "flow data set", "refObjectId": "c6a1f35f-2d09-4f54-8dfb-97e502e1ce92", "uri": "../flows/c6a1f35f-2d09-4f54-8dfb-97e502e1ce92.xml"}, "exchange direction": "INPUT", "other": {"anies": [{"name": "referenceToUnitGroupDataSet", "value": {"shortDescription": [{"value": "kg", "lang": "de"}], "type": "unit group data set", "refObjectId": "ad38d542-3fe9-439d-9b95-2f5f7752acaf", "uri": "../unitgroups/ad38d542-3fe9-439d-9b95-2f5f7752acaf.xml"}}, {"value": "247", "module": "A1-A3"}, {"value": "0", "module": "C3"}, {"value": "0", "module": "C4"}, {"value": "867", "module": "D"}]}, "resolvedFlowVersion": "38.00.000", "flowProperties": [], "typeOfFlow": "Other flow", "classification": {"classHierarchy": "Quantities / Environmental quantities / EPD EN 15804 / LCI indicators", "name": "GaBiCategories"}}, {"dataSetInternalID": 8, "referenceToFlowDataSet": {"shortDescription": [{"value": "Erneuerbare Sekundärbrennstoffe (RSF)", "lang": "de"}, {"value": "Use of renewable secondary fuels (RSF)", "lang": "en"}], "type": "flow data set", "refObjectId": "64333088-a55f-4aa2-9a31-c10b07816787", "uri": "../flows/64333088-a55f-4aa2-9a31-c10b07816787.xml"}, "exchange direction": "INPUT", "other": {"anies": [{"name": "referenceToUnitGroupDataSet", "value": {"shortDescription": [{"value": "MJ", "lang": "de"}], "type": "unit group data set", "refObjectId": "93a60a57-a3c8-11da-a746-0800200c9a66", "uri": "../unitgroups/93a60a57-a3c8-11da-a746-0800200c9a66.xml"}}, {"value": "0", "module": "A1-A3"}, {"value": "0", "module": "C3"}, {"value": "0", "module": "C4"}, {"value": "0", "module": "D"}]}, "resolvedFlowVersion": "38.00.000", "flowProperties": [], "typeOfFlow": "Other flow", "classification": {"classHierarchy": "Quantities / Environmental quantities / EPD EN 15804 / LCI indicators", "name": "GaBiCategories"}}, {"dataSetInternalID": 9, "referenceToFlowDataSet": {"shortDescription": [{"value": "Nicht erneuerbare Sekundärbrennstoffe (NRSF)", "lang": "de"}, {"value": "Use of non renewable secondary fuels (NRSF)", "lang": "en"}], "type": "flow data set", "refObjectId": "89def144-d39a-4287-b86f-efde453ddcb2", "uri": "../flows/89def144-d39a-4287-b86f-efde453ddcb2.xml"}, "exchange direction": "INPUT", "other": {"anies": [{"name": "referenceToUnitGroupDataSet", "value": {"shortDescription": [{"value": "MJ", "lang": "de"}], "type": "unit group data set", "refObjectId": "93a60a57-a3c8-11da-a746-0800200c9a66", "uri": "../unitgroups/93a60a57-a3c8-11da-a746-0800200c9a66.xml"}}, {"value": "0", "module": "A1-A3"}, {"value": "0", "module": "C3"}, {"value": "0", "module": "C4"}, {"value": "0", "module": "D"}]}, "resolvedFlowVersion": "38.00.000", "flowProperties": [], "typeOfFlow": "Other flow", "classification": {"classHierarchy": "Quantities / Environmental quantities / EPD EN 15804 / LCI indicators", "name": "GaBiCategories"}}, {"dataSetInternalID": 10, "referenceToFlowDataSet": {"shortDescription": [{"value": "Einsatz von Süßwasserressourcen (FW)", "lang": "de"}, {"value": "Use of net fresh water (FW)", "lang": "en"}], "type": "flow data set", "refObjectId": "3cf952c8-f3a4-461d-8c96-96456ca62246", "uri": "../flows/3cf952c8-f3a4-461d-8c96-96456ca62246.xml"}, "exchange direction": "INPUT", "other": {"anies": [{"name": "referenceToUnitGroupDataSet", "value": {"shortDescription": [{"value": "m^3", "lang": "de"}], "type": "unit group data set", "refObjectId": "cd950537-0a98-4044-9ba7-9f9a68d0a504", "uri": "../unitgroups/cd950537-0a98-4044-9ba7-9f9a68d0a504.xml"}}, {"value": "2.9", "module": "A1-A3"}, {"value": "0", "module": "C3"}, {"value": "0", "module": "C4"}, {"value": "-1.02", "module": "D"}]}, "resolvedFlowVersion": "38.00.000", "flowProperties": [], "typeOfFlow": "Other flow", "classification": {"classHierarchy": "Quantities / Environmental quantities / EPD EN 15804 / LCI indicators", "name": "GaBiCategories"}}, {"dataSetInternalID": 11, "referenceToFlowDataSet": {"shortDescription": [{"value": "Gefährlicher Abfall zur Deponie (HWD)", "lang": "de"}, {"value": "Hazardous waste disposed (HWD)", "lang": "en"}], "type": "flow data set", "refObjectId": "430f9e0f-59b2-46a0-8e0d-55e0e84948fc", "uri": "../flows/430f9e0f-59b2-46a0-8e0d-55e0e84948fc.xml"}, "exchange direction": "OUTPUT", "other": {"anies": [{"name": "referenceToUnitGroupDataSet", "value": {"shortDescription": [{"value": "kg", "lang": "de"}], "type": "unit group data set", "refObjectId": "ad38d542-3fe9-439d-9b95-2f5f7752acaf", "uri": "../unitgroups/ad38d542-3fe9-439d-9b95-2f5f7752acaf.xml"}}, {"value": "0.00106", "module": "A1-A3"}, {"value": "0", "module": "C3"}, {"value": "0", "module": "C4"}, {"value": "-0.000968", "module": "D"}]}, "resolvedFlowVersion": "38.00.000", "flowProperties": [], "typeOfFlow": "Other flow", "classification": {"classHierarchy": "Quantities / Environmental quantities / EPD EN 15804 / LCI indicators", "name": "GaBiCategories"}}, {"dataSetInternalID": 12, "referenceToFlowDataSet": {"shortDescription": [{"value": "Entsorgter nicht gefährlicher Abfall (NHWD)", "lang": "de"}, {"value": "Non hazardous waste disposed (NHWD)", "lang": "en"}], "type": "flow data set", "refObjectId": "b29ef66b-e286-4afa-949f-62f1a7b4d7fa", "uri": "../flows/b29ef66b-e286-4afa-949f-62f1a7b4d7fa.xml"}, "exchange direction": "OUTPUT", "other": {"anies": [{"name": "referenceToUnitGroupDataSet", "value": {"shortDescription": [{"value": "kg", "lang": "de"}], "type": "unit group data set", "refObjectId": "ad38d542-3fe9-439d-9b95-2f5f7752acaf", "uri": "../unitgroups/ad38d542-3fe9-439d-9b95-2f5f7752acaf.xml"}}, {"value": "26.9", "module": "A1-A3"}, {"value": "0", "module": "C3"}, {"value": "0", "module": "C4"}, {"value": "-23", "module": "D"}]}, "resolvedFlowVersion": "38.00.000", "flowProperties": [], "typeOfFlow": "Other flow", "classification": {"classHierarchy": "Quantities / Environmental quantities / EPD EN 15804 / LCI indicators", "name": "GaBiCategories"}}, {"dataSetInternalID": 13, "referenceToFlowDataSet": {"shortDescription": [{"value": "Entsorgter radioaktiver Abfall (RWD)", "lang": "de"}, {"value": "Radioactive waste disposed (RWD)", "lang": "en"}], "type": "flow data set", "refObjectId": "3449546e-52ad-4b39-b809-9fb77cea8ff6", "uri": "../flows/3449546e-52ad-4b39-b809-9fb77cea8ff6.xml"}, "exchange direction": "OUTPUT", "other": {"anies": [{"name": "referenceToUnitGroupDataSet", "value": {"shortDescription": [{"value": "kg", "lang": "de"}], "type": "unit group data set", "refObjectId": "ad38d542-3fe9-439d-9b95-2f5f7752acaf", "uri": "../unitgroups/ad38d542-3fe9-439d-9b95-2f5f7752acaf.xml"}}, {"value": "0.162", "module": "A1-A3"}, {"value": "0", "module": "C3"}, {"value": "0", "module": "C4"}, {"value": "0.176", "module": "D"}]}, "resolvedFlowVersion": "38.00.000", "flowProperties": [], "typeOfFlow": "Other flow", "classification": {"classHierarchy": "Quantities / Environmental quantities / EPD EN 15804 / LCI indicators", "name": "GaBiCategories"}}, {"dataSetInternalID": 14, "referenceToFlowDataSet": {"shortDescription": [{"value": "Komponenten für die Wiederverwendung (CRU)", "lang": "de"}, {"value": "Components for re-use (CRU)", "lang": "en"}], "type": "flow data set", "refObjectId": "a2b32f97-3fc7-4af2-b209-525bc6426f33", "uri": "../flows/a2b32f97-3fc7-4af2-b209-525bc6426f33.xml"}, "exchange direction": "OUTPUT", "other": {"anies": [{"name": "referenceToUnitGroupDataSet", "value": {"shortDescription": [{"value": "kg", "lang": "de"}], "type": "unit group data set", "refObjectId": "ad38d542-3fe9-439d-9b95-2f5f7752acaf", "uri": "../unitgroups/ad38d542-3fe9-439d-9b95-2f5f7752acaf.xml"}}, {"value": "0", "module": "A1-A3"}, {"value": "0", "module": "C3"}, {"value": "0", "module": "C4"}, {"value": "60.7", "module": "D"}]}, "resolvedFlowVersion": "38.00.000", "flowProperties": [], "typeOfFlow": "Other flow", "classification": {"classHierarchy": "Quantities / Environmental quantities / EPD EN 15804 / LCI indicators", "name": "GaBiCategories"}}, {"dataSetInternalID": 15, "referenceToFlowDataSet": {"shortDescription": [{"value": "Stoffe zum Recycling (MFR)", "lang": "de"}, {"value": "Materials for recycling (MFR)", "lang": "en"}], "type": "flow data set", "refObjectId": "d7fe48a5-4103-49c8-9aae-b0b5dfdbd6ae", "uri": "../flows/d7fe48a5-4103-49c8-9aae-b0b5dfdbd6ae.xml"}, "exchange direction": "OUTPUT", "other": {"anies": [{"name": "referenceToUnitGroupDataSet", "value": {"shortDescription": [{"value": "kg", "lang": "de"}], "type": "unit group data set", "refObjectId": "ad38d542-3fe9-439d-9b95-2f5f7752acaf", "uri": "../unitgroups/ad38d542-3fe9-439d-9b95-2f5f7752acaf.xml"}}, {"value": "146", "module": "A1-A3"}, {"value": "0", "module": "C3"}, {"value": "0", "module": "C4"}, {"value": "867", "module": "D"}]}, "resolvedFlowVersion": "38.00.000", "flowProperties": [], "typeOfFlow": "Other flow", "classification": {"classHierarchy": "Quantities / Environmental quantities / EPD EN 15804 / LCI indicators", "name": "GaBiCategories"}}, {"dataSetInternalID": 16, "referenceToFlowDataSet": {"shortDescription": [{"value": "Stoffe für die Energierückgewinnung (MER)", "lang": "de"}, {"value": "Materials for energy recovery (MER)", "lang": "en"}], "type": "flow data set", "refObjectId": "59a9181c-3aaf-46ee-8b13-2b3723b6e447", "uri": "../flows/59a9181c-3aaf-46ee-8b13-2b3723b6e447.xml"}, "exchange direction": "OUTPUT", "other": {"anies": [{"name": "referenceToUnitGroupDataSet", "value": {"shortDescription": [{"value": "kg", "lang": "de"}], "type": "unit group data set", "refObjectId": "ad38d542-3fe9-439d-9b95-2f5f7752acaf", "uri": "../unitgroups/ad38d542-3fe9-439d-9b95-2f5f7752acaf.xml"}}, {"value": "0", "module": "A1-A3"}, {"value": "0", "module": "C3"}, {"value": "0", "module": "C4"}, {"value": "0", "module": "D"}]}, "resolvedFlowVersion": "38.00.000", "flowProperties": [], "typeOfFlow": "Other flow", "classification": {"classHierarchy": "Quantities / Environmental quantities / EPD EN 15804 / LCI indicators", "name": "GaBiCategories"}}, {"dataSetInternalID": 17, "referenceToFlowDataSet": {"shortDescription": [{"value": "Exportierte elektrische Energie (EEE)", "lang": "de"}, {"value": "Exported electrical energy (EEE)", "lang": "en"}], "type": "flow data set", "refObjectId": "4da0c987-2b76-40d6-9e9e-82a017aaaf29", "uri": "../flows/4da0c987-2b76-40d6-9e9e-82a017aaaf29.xml"}, "exchange direction": "OUTPUT", "other": {"anies": [{"name": "referenceToUnitGroupDataSet", "value": {"shortDescription": [{"value": "MJ", "lang": "de"}], "type": "unit group data set", "refObjectId": "93a60a57-a3c8-11da-a746-0800200c9a66", "uri": "../unitgroups/93a60a57-a3c8-11da-a746-0800200c9a66.xml"}}, {"value": "0", "module": "A1-A3"}, {"value": "0", "module": "C3"}, {"value": "0", "module": "C4"}, {"value": "0", "module": "D"}]}, "resolvedFlowVersion": "38.00.000", "flowProperties": [], "typeOfFlow": "Other flow", "classification": {"classHierarchy": "Quantities / Environmental quantities / EPD EN 15804 / LCI indicators", "name": "GaBiCategories"}}, {"dataSetInternalID": 18, "referenceToFlowDataSet": {"shortDescription": [{"value": "Exportierte thermische Energie (EET)", "lang": "de"}, {"value": "Exported thermal energy (EET)", "lang": "en"}], "type": "flow data set", "refObjectId": "98daf38a-7a79-46d3-9a37-2b7bd0955810", "uri": "../flows/98daf38a-7a79-46d3-9a37-2b7bd0955810.xml"}, "exchange direction": "OUTPUT", "other": {"anies": [{"name": "referenceToUnitGroupDataSet", "value": {"shortDescription": [{"value": "MJ", "lang": "de"}], "type": "unit group data set", "refObjectId": "93a60a57-a3c8-11da-a746-0800200c9a66", "uri": "../unitgroups/93a60a57-a3c8-11da-a746-0800200c9a66.xml"}}, {"value": "0", "module": "A1-A3"}, {"value": "0", "module": "C3"}, {"value": "0", "module": "C4"}, {"value": "0", "module": "D"}]}, "resolvedFlowVersion": "38.00.000", "flowProperties": [], "typeOfFlow": "Other flow", "classification": {"classHierarchy": "Quantities / Environmental quantities / EPD EN 15804 / LCI indicators", "name": "GaBiCategories"}}]}, "LCIAResults": {"LCIAResult": [{"referenceToLCIAMethodDataSet": {"shortDescription": [{"value": "Globales Erwärmungspotenzial total (GWP-total)", "lang": "de"}, {"value": "Global Warming Potential total (GWP-total)", "lang": "en"}], "type": "LCIA method data set", "refObjectId": "6a37f984-a4b3-458a-a20a-64418c145fa2", "uri": "../lciamethods/6a37f984-a4b3-458a-a20a-64418c145fa2.xml"}, "other": {"anies": [{"name": "referenceToUnitGroupDataSet", "value": {"shortDescription": [{"value": "kg CO_(2)-Äq.", "lang": "de"}], "type": "unit group data set", "refObjectId": "1ebf3012-d0db-4de2-aefd-ef30cedb0be1", "uri": "../unitgroups/1ebf3012-d0db-4de2-aefd-ef30cedb0be1.xml"}}, {"value": "2280", "module": "A1-A3"}, {"value": "0", "module": "C3"}, {"value": "0", "module": "C4"}, {"value": "-1530", "module": "D"}]}}, {"referenceToLCIAMethodDataSet": {"shortDescription": [{"value": "Globales Erwärmungspotenzial fossil (GWP-fossil)", "lang": "de"}, {"value": "Global Warming Potential fossil fuels (GWP-fossil)", "lang": "en"}], "type": "LCIA method data set", "refObjectId": "5f635281-343e-44fb-83df-1971b155e6b6", "uri": "../lciamethods/5f635281-343e-44fb-83df-1971b155e6b6.xml"}, "other": {"anies": [{"name": "referenceToUnitGroupDataSet", "value": {"shortDescription": [{"value": "kg CO_(2)-Äq.", "lang": "de"}], "type": "unit group data set", "refObjectId": "1ebf3012-d0db-4de2-aefd-ef30cedb0be1", "uri": "../unitgroups/1ebf3012-d0db-4de2-aefd-ef30cedb0be1.xml"}}, {"value": "2280", "module": "A1-A3"}, {"value": "0", "module": "C3"}, {"value": "0", "module": "C4"}, {"value": "-1530", "module": "D"}]}}, {"referenceToLCIAMethodDataSet": {"shortDescription": [{"value": "Globales Erwärmungspotenzial biogen (GWP-biogenic)", "lang": "de"}, {"value": "Global Warming Potential biogenic (GWP-biogenic)", "lang": "en"}], "type": "LCIA method data set", "refObjectId": "2356e1ab-0185-4db5-86e5-16de51c7485c", "uri": "../lciamethods/2356e1ab-0185-4db5-86e5-16de51c7485c.xml"}, "other": {"anies": [{"name": "referenceToUnitGroupDataSet", "value": {"shortDescription": [{"value": "kg CO_(2)-Äq.", "lang": "de"}], "type": "unit group data set", "refObjectId": "1ebf3012-d0db-4de2-aefd-ef30cedb0be1", "uri": "../unitgroups/1ebf3012-d0db-4de2-aefd-ef30cedb0be1.xml"}}, {"value": "3.56", "module": "A1-A3"}, {"value": "0", "module": "C3"}, {"value": "0", "module": "C4"}, {"value": "1.81", "module": "D"}]}}, {"referenceToLCIAMethodDataSet": {"shortDescription": [{"value": "Globales Erwärmungspotenzial luluc (GWP-luluc)", "lang": "de"}, {"value": "Global Warming Potential luluc (GWP-luluc)", "lang": "en"}], "type": "LCIA method data set", "refObjectId": "4331bbdb-978a-490d-8707-eeb047f01a55", "uri": "../lciamethods/4331bbdb-978a-490d-8707-eeb047f01a55.xml"}, "other": {"anies": [{"name": "referenceToUnitGroupDataSet", "value": {"shortDescription": [{"value": "kg CO_(2)-Äq.", "lang": "de"}], "type": "unit group data set", "refObjectId": "1ebf3012-d0db-4de2-aefd-ef30cedb0be1", "uri": "../unitgroups/1ebf3012-d0db-4de2-aefd-ef30cedb0be1.xml"}}, {"value": "1.19", "module": "A1-A3"}, {"value": "0", "module": "C3"}, {"value": "0", "module": "C4"}, {"value": "-0.255", "module": "D"}]}}, {"referenceToLCIAMethodDataSet": {"shortDescription": [{"value": "Abbau Potential der stratosphärischen Ozonschicht (ODP)", "lang": "de"}, {"value": "Depletion potential of the stratospheric ozone layer (ODP)", "lang": "en"}], "type": "LCIA method data set", "refObjectId": "b5c629d6-def3-11e6-bf01-fe55135034f3", "uri": "../lciamethods/b5c629d6-def3-11e6-bf01-fe55135034f3.xml"}, "other": {"anies": [{"name": "referenceToUnitGroupDataSet", "value": {"shortDescription": [{"value": "kg CFC11-Äq.", "lang": "de"}], "type": "unit group data set", "refObjectId": "d9e957c9-7309-4474-bf3a-7777df6c4e5b", "uri": "../unitgroups/d9e957c9-7309-4474-bf3a-7777df6c4e5b.xml"}}, {"value": "2.88E-08", "module": "A1-A3"}, {"value": "0", "module": "C3"}, {"value": "0", "module": "C4"}, {"value": "-2.65E-08", "module": "D"}]}}, {"referenceToLCIAMethodDataSet": {"shortDescription": [{"value": "Versauerungspotenzial von Boden und Wasser (AP)", "lang": "de"}, {"value": "Acidification potential of land and water (AP)", "lang": "en"}], "type": "LCIA method data set", "refObjectId": "b5c611c6-def3-11e6-bf01-fe55135034f3", "uri": "../lciamethods/b5c611c6-def3-11e6-bf01-fe55135034f3.xml"}, "other": {"anies": [{"name": "referenceToUnitGroupDataSet", "value": {"shortDescription": [{"value": "mol H^(+)-Äq.", "lang": "de"}], "type": "unit group data set", "refObjectId": "42e089ac-92bf-4bf2-8ca1-5fc40d18f2ed", "uri": "../unitgroups/42e089ac-92bf-4bf2-8ca1-5fc40d18f2ed.xml"}}, {"value": "6.09", "module": "A1-A3"}, {"value": "0", "module": "C3"}, {"value": "0", "module": "C4"}, {"value": "-4.47", "module": "D"}]}}, {"referenceToLCIAMethodDataSet": {"shortDescription": [{"value": "Eutrophierungspotenzial Süßwasser (EP-freshwater)", "lang": "de"}, {"value": "Eutrophication potential aquatic freshwater (EP-freshwater)", "lang": "en"}], "type": "LCIA method data set", "refObjectId": "b53ec18f-7377-4ad3-86eb-cc3f4f276b2b", "uri": "../lciamethods/b53ec18f-7377-4ad3-86eb-cc3f4f276b2b.xml"}, "other": {"anies": [{"name": "referenceToUnitGroupDataSet", "value": {"shortDescription": [{"value": "kg PO_(4)-Äq.", "lang": "de"}], "type": "unit group data set", "refObjectId": "0429039d-a61d-4590-ba67-aa4a20a810a1", "uri": "../unitgroups/0429039d-a61d-4590-ba67-aa4a20a810a1.xml"}}, {"value": "0.00206", "module": "A1-A3"}, {"value": "0", "module": "C3"}, {"value": "0", "module": "C4"}, {"value": "-0.000473", "module": "D"}]}}, {"referenceToLCIAMethodDataSet": {"shortDescription": [{"value": "Eutrophierungspotenzial Salzwasser (EP-marine)", "lang": "de"}, {"value": "Eutrophication potential aquatic marine (EP-marine)", "lang": "en"}], "type": "LCIA method data set", "refObjectId": "b5c619fa-def3-11e6-bf01-fe55135034f3", "uri": "../lciamethods/b5c619fa-def3-11e6-bf01-fe55135034f3.xml"}, "other": {"anies": [{"name": "referenceToUnitGroupDataSet", "value": {"shortDescription": [{"value": "kg N-Äq.", "lang": "de"}], "type": "unit group data set", "refObjectId": "d05bb823-ecdf-4686-8c40-bf1d9257859f", "uri": "../unitgroups/d05bb823-ecdf-4686-8c40-bf1d9257859f.xml"}}, {"value": "1.29", "module": "A1-A3"}, {"value": "0", "module": "C3"}, {"value": "0", "module": "C4"}, {"value": "-0.857", "module": "D"}]}}, {"referenceToLCIAMethodDataSet": {"shortDescription": [{"value": "Eutrophierungspotenzial Land (EP-terrestrial)", "lang": "de"}, {"value": "Eutrophication potential terrestrial (EP-terrestrial)", "lang": "en"}], "type": "LCIA method data set", "refObjectId": "b5c614d2-def3-11e6-bf01-fe55135034f3", "uri": "../lciamethods/b5c614d2-def3-11e6-bf01-fe55135034f3.xml"}, "other": {"anies": [{"name": "referenceToUnitGroupDataSet", "value": {"shortDescription": [{"value": "mol N-Äq.", "lang": "de"}], "type": "unit group data set", "refObjectId": "71b4d617-0ec9-4d3f-b65e-e438940c2401", "uri": "../unitgroups/71b4d617-0ec9-4d3f-b65e-e438940c2401.xml"}}, {"value": "14", "module": "A1-A3"}, {"value": "0", "module": "C3"}, {"value": "0", "module": "C4"}, {"value": "-9.31", "module": "D"}]}}, {"referenceToLCIAMethodDataSet": {"shortDescription": [{"value": "Bildungspotential für troposphärisches Ozon (POCP)", "lang": "de"}, {"value": "Formation potential of tropospheric ozone photochemical oxidants (POCP)", "lang": "en"}], "type": "LCIA method data set", "refObjectId": "b5c610fe-def3-11e6-bf01-fe55135034f3", "uri": "../lciamethods/b5c610fe-def3-11e6-bf01-fe55135034f3.xml"}, "other": {"anies": [{"name": "referenceToUnitGroupDataSet", "value": {"shortDescription": [{"value": "kg NMVOC-Äq.", "lang": "de"}], "type": "unit group data set", "refObjectId": "d27c25f8-fbc1-44c6-b47b-4adbae4199c6", "uri": "../unitgroups/d27c25f8-fbc1-44c6-b47b-4adbae4199c6.xml"}}, {"value": "3.73", "module": "A1-A3"}, {"value": "0", "module": "C3"}, {"value": "0", "module": "C4"}, {"value": "-2.29", "module": "D"}]}}, {"referenceToLCIAMethodDataSet": {"shortDescription": [{"value": "Potenzial für den abiotischen Abbau nicht fossiler Ressourcen (ADPE)", "lang": "de"}, {"value": "Abiotic depletion potential for non fossil resources (ADPE)", "lang": "en"}], "type": "LCIA method data set", "refObjectId": "b2ad6494-c78d-11e6-9d9d-cec0c932ce01", "uri": "../lciamethods/b2ad6494-c78d-11e6-9d9d-cec0c932ce01.xml"}, "other": {"anies": [{"name": "referenceToUnitGroupDataSet", "value": {"shortDescription": [{"value": "kg Sb-Äq.", "lang": "de"}], "type": "unit group data set", "refObjectId": "54ccd2d9-a32a-4fc2-923d-f2c8c93e89d4", "uri": "../unitgroups/54ccd2d9-a32a-4fc2-923d-f2c8c93e89d4.xml"}}, {"value": "0.000455", "module": "A1-A3"}, {"value": "0", "module": "C3"}, {"value": "0", "module": "C4"}, {"value": "-0.000255", "module": "D"}]}}, {"referenceToLCIAMethodDataSet": {"shortDescription": [{"value": "Potenzial für den abiotischen Abbau fossiler Brennstoffe (ADPF)", "lang": "de"}, {"value": "Abiotic depletion potential for fossil resources (ADPF)", "lang": "en"}], "type": "LCIA method data set", "refObjectId": "b2ad6110-c78d-11e6-9d9d-cec0c932ce01", "uri": "../lciamethods/b2ad6110-c78d-11e6-9d9d-cec0c932ce01.xml"}, "other": {"anies": [{"name": "referenceToUnitGroupDataSet", "value": {"shortDescription": [{"value": "MJ", "lang": "de"}], "type": "unit group data set", "refObjectId": "93a60a57-a3c8-11da-a746-0800200c9a66", "uri": "../unitgroups/93a60a57-a3c8-11da-a746-0800200c9a66.xml"}}, {"value": "22000", "module": "A1-A3"}, {"value": "0", "module": "C3"}, {"value": "0", "module": "C4"}, {"value": "-12600", "module": "D"}]}}, {"referenceToLCIAMethodDataSet": {"shortDescription": [{"value": "Wassernutzung (WDP)", "lang": "de"}, {"value": "Water use (WDP)", "lang": "en"}], "type": "LCIA method data set", "refObjectId": "b2ad66ce-c78d-11e6-9d9d-cec0c932ce01", "uri": "../lciamethods/b2ad66ce-c78d-11e6-9d9d-cec0c932ce01.xml"}, "other": {"anies": [{"name": "referenceToUnitGroupDataSet", "value": {"shortDescription": [{"value": "m^(3) Welt-Äq. entzogen", "lang": "de"}], "type": "unit group data set", "refObjectId": "6ae2df01-888e-46c8-b17d-49fa3869b476", "uri": "../unitgroups/6ae2df01-888e-46c8-b17d-49fa3869b476.xml"}}, {"value": "3.79", "module": "A1-A3"}, {"value": "0", "module": "C3"}, {"value": "0", "module": "C4"}, {"value": "-0.524", "module": "D"}]}}, {"referenceToLCIAMethodDataSet": {"shortDescription": [{"value": "Auftreten von Krankheiten aufgrund von Feinstaubemissionen (PM)", "lang": "de"}, {"value": "Incidence of disease due to PM emissions (PM)", "lang": "en"}], "type": "LCIA method data set", "refObjectId": "b5c602c6-def3-11e6-bf01-fe55135034f3", "uri": "../lciamethods/b5c602c6-def3-11e6-bf01-fe55135034f3.xml"}, "other": {"anies": [{"name": "referenceToUnitGroupDataSet", "value": {"shortDescription": [{"value": "Krankheitsfälle", "lang": "de"}], "type": "unit group data set", "refObjectId": "3883559b-648f-4afc-8ba2-0bd24f3affa3", "uri": "../unitgroups/3883559b-648f-4afc-8ba2-0bd24f3affa3.xml"}}, {"module": "A1-A3"}, {"module": "C3"}, {"module": "C4"}, {"module": "D"}]}}, {"referenceToLCIAMethodDataSet": {"shortDescription": [{"value": "Wirkung durch Exposition des Menschen mit U235 (IR)", "lang": "de"}, {"value": "Human exposure efficiency relative to U235 (IR)", "lang": "en"}], "type": "LCIA method data set", "refObjectId": "b5c632be-def3-11e6-bf01-fe55135034f3", "uri": "../lciamethods/b5c632be-def3-11e6-bf01-fe55135034f3.xml"}, "other": {"anies": [{"name": "referenceToUnitGroupDataSet", "value": {"shortDescription": [{"value": "kBq U235-Äq.", "lang": "de"}], "type": "unit group data set", "refObjectId": "456b05bf-1415-44a9-9993-02452f554c09", "uri": "../unitgroups/456b05bf-1415-44a9-9993-02452f554c09.xml"}}, {"module": "A1-A3"}, {"module": "C3"}, {"module": "C4"}, {"module": "D"}]}}, {"referenceToLCIAMethodDataSet": {"shortDescription": [{"value": "Toxizitätsvergleichseinheit für Ökosysteme (ETP-fw)", "lang": "de"}, {"value": "Comparative toxic unit for ecosystems (ETP-fw)", "lang": "en"}], "type": "LCIA method data set", "refObjectId": "ee1082d1-b0f7-43ca-a1f0-21e2a4a74511", "uri": "../lciamethods/ee1082d1-b0f7-43ca-a1f0-21e2a4a74511.xml"}, "other": {"anies": [{"name": "referenceToUnitGroupDataSet", "value": {"shortDescription": [{"value": "CTUe", "lang": "de"}], "type": "unit group data set", "refObjectId": "aa959ded-f1eb-4efb-9c5c-2d60be36b3e6", "uri": "../unitgroups/aa959ded-f1eb-4efb-9c5c-2d60be36b3e6.xml"}}, {"module": "A1-A3"}, {"module": "C3"}, {"module": "C4"}, {"module": "D"}]}}, {"referenceToLCIAMethodDataSet": {"shortDescription": [{"value": "Toxizitätsvergleichseinheit für Menschen (krebserregend) (HTP-c)", "lang": "de"}, {"value": "Comparative toxic unit for humans (carcinogenic) (HTP-c)", "lang": "en"}], "type": "LCIA method data set", "refObjectId": "2299222a-bbd8-474f-9d4f-4dd1f18aea7c", "uri": "../lciamethods/2299222a-bbd8-474f-9d4f-4dd1f18aea7c.xml"}, "other": {"anies": [{"name": "referenceToUnitGroupDataSet", "value": {"shortDescription": [{"value": "CTUh", "lang": "de"}], "type": "unit group data set", "refObjectId": "d4c9523e-2d7e-49fd-8469-998f547d3a70", "uri": "../unitgroups/d4c9523e-2d7e-49fd-8469-998f547d3a70.xml"}}, {"module": "A1-A3"}, {"module": "C3"}, {"module": "C4"}, {"module": "D"}]}}, {"referenceToLCIAMethodDataSet": {"shortDescription": [{"value": "Toxizitätsvergleichseinheit für Menschen (nicht krebserregend) (HTP-nc)", "lang": "de"}, {"value": "Comparative toxic unit for humans (noncarcinogenic) (HTP-nc)", "lang": "en"}], "type": "LCIA method data set", "refObjectId": "3af763a5-b7a1-48c9-9cee-1f223481fcef", "uri": "../lciamethods/3af763a5-b7a1-48c9-9cee-1f223481fcef.xml"}, "other": {"anies": [{"name": "referenceToUnitGroupDataSet", "value": {"shortDescription": [{"value": "CTUh", "lang": "de"}], "type": "unit group data set", "refObjectId": "d4c9523e-2d7e-49fd-8469-998f547d3a70", "uri": "../unitgroups/d4c9523e-2d7e-49fd-8469-998f547d3a70.xml"}}, {"module": "A1-A3"}, {"module": "C3"}, {"module": "C4"}, {"module": "D"}]}}, {"referenceToLCIAMethodDataSet": {"shortDescription": [{"value": "Bodenqualitätsindex (SQP)", "lang": "de"}, {"value": "Soil quality index (SQP)", "lang": "en"}], "type": "LCIA method data set", "refObjectId": "b2ad6890-c78d-11e6-9d9d-cec0c932ce01", "uri": "../lciamethods/b2ad6890-c78d-11e6-9d9d-cec0c932ce01.xml"}, "other": {"anies": [{"name": "referenceToUnitGroupDataSet", "value": {"shortDescription": [{"value": "SQP", "lang": "de"}], "type": "unit group data set", "refObjectId": "f130951c-e67f-4f7f-8dd4-665de3974e18", "uri": "../unitgroups/f130951c-e67f-4f7f-8dd4-665de3974e18.xml"}}, {"module": "A1-A3"}, {"module": "C3"}, {"module": "C4"}, {"module": "D"}]}}]}, "otherAttributes": {"{http://www.indata.network/EPD/2019}epd-version": "1.2"}, "version": "1.1", "locations": "../ILCDLocations.xml"}