{"processInformation": {"dataSetInformation": {"UUID": "ba58d8b9-945b-4428-b4e0-aecda8b3df18", "name": {"baseName": [{"value": "Insulated glazing, triple pane", "lang": "en"}, {"value": "Dreifachverglasung", "lang": "de"}], "functionalUnitFlowProperties": [{"value": "31 kg/m2", "lang": "en"}]}, "classificationInformation": {"classification": [{"class": [{"value": "Komponenten von Fenstern und Vorhangfassaden", "level": 0, "classId": "7"}, {"value": "Füllungen", "level": 1, "classId": "7.2"}, {"value": "Transparente Füllungen", "level": 2, "classId": "7.2.01"}], "name": "oekobau.dat"}]}, "generalComment": [{"value": "This data set has been modeled according to the European Standard EN 15804+A2 for Sustainable Building. Results are depicted in modules that allow the structured expression of results over the entire life cycle.", "lang": "en"}, {"value": "Dieser Datensatz wurde nach dem European Standard EN 15804+A2 für Nachhaltiges Bauen modelliert. Ergebnisse werden in Modulen abgebildet, die den strukturierten Ausdruck von Ergebnissen über den gesamten Lebenszyklus zulassen.", "lang": "de"}], "other": {"anies": [{"margins": 20, "description": [{"value": "Product system depicted except for a few missing processes / flows. Technological, temporal and geographic representativeness partly given.", "lang": "en"}, {"value": "Produktsystem bis auf wenige Prozesse/Flüsse abgebildet. Technologische, zeitliche und geographische Repräsentativität teilweise gegeben.", "lang": "de"}]}]}}, "quantitativeReference": {"referenceToReferenceFlow": [100551], "type": "Reference flow(s)"}, "time": {"referenceYear": 2023, "dataSetValidUntil": 2026, "timeRepresentativenessDescription": [{"value": "Annual average", "lang": "en"}, {"value": "Jährlicher Durchschnitt", "lang": "de"}]}, "geography": {"locationOfOperationSupplyOrProduction": {"descriptionOfRestrictions": [{"value": "The data set represents the country specific situation in Germany, focusing on the main technologies, the region specific characteristics and / or import statistics.", "lang": "en"}, {"value": "Der Datensatz bildet die länderspezifische Situation in Deutschland ab. Dabei werden Haupttechnologien, spezifische regionale Charakteristiken und ggf. Importstatistiken berücksichtigt.", "lang": "de"}], "location": "DE"}}, "technology": {"technologyDescriptionAndIncludedProcesses": [{"value": "Foreground system:\nThe system boundaries comprise the cradle to gate life cycle of 1m2 of three panes insulation glas without fixing system or frame. The LCI dataset consider the production and assembly of the of the glas panes parts and the side materials (sealing materials, spacers, argon, surface treatment of the glass). Reference product scaled to 1m² Based on 3 sheet glass of 124cm*  99cm, 3 panes of 4mm thick, 2  panes treated (low emission coating) 16mm between panes. \nSealing, spacer and argon (between each pane)Transportation processes for the raw materials are accounted for as far as data on average transport distances were available. All relevant energy and energy flow are included in the system. Life cycle impacts of production equipment and infrastructure were not included in the system as no evidence could be justified that these are to any extent relevant and thus fell under the cut-off criteria. In mass production the impact of production equipment and infrastructure normally is in orders of magnitude lower than the impacts of material and energy supply.\n\nIn module C1, a manual dismantling (no loads) is assumed, collecting losses are neglected.\nThe transport in module C2 to the recycling plant takes place with a truck (50km).\n\nTratment of metal components:\nCollecting losses are neglected. It is assumed that all metals reach the end of the waste status immediately after dismantling. This means that the loads for processing and the credits for the substitution of primary material are shown in Module D.\nModule D includes loads for sorting, remelting, slag treatment, landfill, filtration of dusts and dross treatment. Credits are given for the net scrap amount (amount returned minus secondary material content, minus processing losses) for the average material mix (from different alloys).\n\nTreatment of plastic components:\nModule C3 takes into account the grinding and thermal treatment (combustion) of the material. When calculating combustion emissions and credits, the specific calorific value of each material and the material composition are taken into account.\nIn module D credits for the substitution of electricity (German electricity mix) and thermal energy (from natural gas) are given.\n\nTreatment of renewable raw materials:\nModule C3 takes into account the grinding and thermal treatment (combustion) of the material. It is assumed that the material reaches the end of the waste status immediately after dismantling. The CO2 absorbed and stored in the material by photosynthesis (from module A1) is written off in C3 (CO2 neutrality within the product system according to EN 16485: Round and sawn timber - Environmental Product Declarations - Product category rules for wood and wood-based products for use in construction, 2014).\nModule D contains the loads through the operation of the recovery facility (excluding biogenic CO2, see above) and credits for the substitution of electricity (German electricity mix) and thermal energy (from natural gas). The calculation of combustion emissions and credits takes into account the specific calorific value of the material and the material composition.\n\nTreatment of inert material components:\nIn module C4 the average landfill emissions corresponding to the product (reference country Germany) are shown. The use of landfill gas is not taken into account.", "lang": "en"}, {"value": "Dieser Datensatz beschreibt die Herstellung und Entsorgung einer 3- Scheiben- Isolierverglasung ohne Befestigungssystem oder Rahmen. Die Verglasung besteht aus 3 Scheiben (Floatglas) mit jeweils 4mm Dicke, zweifach beschichtet (low-e) und 16mm Abstand zwischen den Scheiben. Im Scheibenzwischenraum befindet sich eine Argonfüllung. Der U-Wert der Verglasung beträgt 0,7 W/m²*K. Der LCI- Datensatz berücksichtigt die Herstellung und die Montage der Glasscheiben und des Randverbundes (Dichtungsmaterialien, Distanzstück (warm edge), Argonfüllung und Oberflächenbehandlung des Glases). Das Referenzprodukt ist auf 1m² skaliert. Es basiert auf einer Dreifachverglasung mit den Abmessungen 124cm* 99cm.\n\nTransportprozesse für die Rohstoffe wurden berücksichtigt. Alle wichtigen Energie- und Stoffflüsse sind im System inbegriffen. Die Wirkungsbilanz der Produktionsanlagen und der Infrastruktur wurde im System nicht berücksichtigt.\n\nIn der Entsorgungsphase wird ein manueller Rückbau (lastenfrei) in Modul C1 angenommen. Der Transport in Modul C2 zur Deponie erfolgt mit einem LKW (50km). In C3 wird, sofern relevant, eine Verpackung mit PE-Folie berücksichtigt (z.B. bei Mineralfaserprodukten, 0,0125 kg Folie je kg entsorgtes Material). In Modul C4 werden dem Produkt entsprechende, durchschnittliche Deponieemissionen (Bezugsraum Deutschland) ausgewiesen. Die Nutzung von Deponiegas wird nicht berücksichtigt.\n\nWenden Sie diesen Datensatz an, indem Sie die Fläche der Dreifachisolierverglasung in m² mit dem Ergebnis dieses Datensatzes multiplizieren.", "lang": "de"}], "technologicalApplicability": [{"value": "This product can be used in construction.", "lang": "en"}, {"value": "Dieses Produkt kann im Baubereich verwendet werden.", "lang": "de"}], "referenceToTechnologyFlowDiagrammOrPicture": [{"shortDescription": [{"value": "construction_three panes insulation glass.jpg", "lang": "en"}], "type": "source data set", "refObjectId": "32e7da00-afb7-4cb6-9ab5-c4f7a5212020", "version": "24.01.000", "uri": "../sources/32e7da00-afb7-4cb6-9ab5-c4f7a5212020.xml"}]}}, "modellingAndValidation": {"LCIMethodAndAllocation": {"typeOfDataSet": "EPD", "other": {"anies": [{"name": "subType", "value": "generic dataset"}]}}, "dataSourcesTreatmentAndRepresentativeness": {"referenceToDataSource": [{"shortDescription": [{"value": "Documentation of data quality management", "lang": "en"}], "type": "source data set", "refObjectId": "e3bd9bbf-2c3c-42aa-8892-fd13f1065ca5", "version": "24.01.000", "uri": "../sources/e3bd9bbf-2c3c-42aa-8892-fd13f1065ca5.xml"}, {"shortDescription": [{"value": "GaBi Database Edition 2021, CUP2021.01", "lang": "en"}], "type": "source data set", "refObjectId": "1cece811-7501-44d4-8067-9259bd5cb835", "version": "00.01.000", "uri": "../sources/1cece811-7501-44d4-8067-9259bd5cb835.xml"}, {"shortDescription": [{"value": "Sphera Managed LCA Content Databases (all versions)", "lang": "en"}], "type": "source data set", "refObjectId": "28d74cc0-db8b-4d7e-bc44-5f6d56ce0c4a", "version": "00.03.002", "uri": "../sources/28d74cc0-db8b-4d7e-bc44-5f6d56ce0c4a.xml"}], "useAdviceForDataSet": [{"value": "The data set represents a cradle to gate inventory. It can be used to characterise the supply chain situation of the respective commodity in a representative manner. Combination with individual unit processes using this commodity enables the generation of user-specific (product) LCAs.", "lang": "en"}, {"value": "Der Datensatz repräsentiert ein Cradle to Gate Inventar. Er kann verwendet werden, um die Lieferkette des jeweiligen Produktes in einer repräsentativen Weise zu charakterisieren. Die Kombination mit einzelnen Einheitenprozessen und diesem Produkt ermöglicht die Erstellung von anwenderspezifischen (Produkt-) LCAs.", "lang": "de"}]}, "validation": {"review": [{"referenceToNameOfReviewerAndInstitution": [{"shortDescription": [{"value": "Sphera Solutions GmbH", "lang": "en"}], "type": "contact data set", "refObjectId": "d7fa0337-f279-430d-becf-7f3111a85010", "version": "24.01.000", "uri": "../contacts/d7fa0337-f279-430d-becf-7f3111a85010.xml"}], "type": "Dependent internal review"}, {"referenceToNameOfReviewerAndInstitution": [{"shortDescription": [{"value": "Sphera Product Sustainability user forum", "lang": "en"}], "type": "contact data set", "refObjectId": "8f1306f0-7b83-4f36-a537-aa83f0498266", "version": "24.01.000", "uri": "../contacts/8f1306f0-7b83-4f36-a537-aa83f0498266.xml"}], "type": "Independent external review"}]}, "complianceDeclarations": {"compliance": [{"referenceToComplianceSystem": {"shortDescription": [{"value": "EN 15804+A2 (EF 3.1)", "lang": "de"}, {"value": "EN 15804+A2 (EF 3.1)", "lang": "en"}], "type": "source data set", "refObjectId": "d4aa3ec7-b1d7-4a4a-a6cb-37af88dcc902", "version": "00.01.000", "uri": "../sources/d4aa3ec7-b1d7-4a4a-a6cb-37af88dcc902.xml"}, "approvalOfOverallCompliance": "Fully compliant"}]}}, "administrativeInformation": {"dataGenerator": {"referenceToPersonOrEntityGeneratingTheDataSet": [{"shortDescription": [{"value": "Sphera Solutions GmbH", "lang": "en"}], "type": "contact data set", "refObjectId": "d7fa0337-f279-430d-becf-7f3111a85010", "version": "24.01.000", "uri": "../contacts/d7fa0337-f279-430d-becf-7f3111a85010.xml"}]}, "dataEntryBy": {"timeStamp": 1718121636000, "referenceToDataSetFormat": [{"shortDescription": [{"value": "ILCD format 1.1", "lang": "de"}, {"value": "ILCD format 1.1", "lang": "en"}], "type": "source data set", "refObjectId": "a97a0155-0234-4b87-b4ce-a45da52f2a40", "version": "01.00.000", "uri": "../sources/a97a0155-0234-4b87-b4ce-a45da52f2a40.xml"}, {"shortDescription": [{"value": "EPD-Datenformaterweiterungen v1.2", "lang": "de"}, {"value": "EPD Data Format Extensions v1.2", "lang": "en"}], "type": "source data set", "refObjectId": "a29449fd-aa2f-4de8-b5d7-4b06b43c6fde", "version": "00.01.000", "uri": "../sources/a29449fd-aa2f-4de8-b5d7-4b06b43c6fde.xml"}], "referenceToPersonOrEntityEnteringTheData": {"shortDescription": [{"value": "Sphera Solutions GmbH", "lang": "en"}], "type": "contact data set", "refObjectId": "d7fa0337-f279-430d-becf-7f3111a85010", "version": "24.01.000", "uri": "../contacts/d7fa0337-f279-430d-becf-7f3111a85010.xml"}}, "publicationAndOwnership": {"dataSetVersion": "20.24.070", "referenceToPrecedingDataSetVersion": [{"shortDescription": [{"value": "Insulated glazing, triple pane", "lang": "en"}], "type": "process data set", "refObjectId": "6eaddefb-7a0f-43e4-a0cb-8459c26e0947", "uri": "https://www.oekobaudat.de/OEKOBAU.DAT/resource/processes/6eaddefb-7a0f-43e4-a0cb-8459c26e0947?version=20.23.050"}], "referenceToRegistrationAuthority": {"shortDescription": [{"value": "Sphera Solutions GmbH", "lang": "en"}], "type": "contact data set", "refObjectId": "d7fa0337-f279-430d-becf-7f3111a85010", "version": "24.01.000", "uri": "../contacts/d7fa0337-f279-430d-becf-7f3111a85010.xml"}, "referenceToOwnershipOfDataSet": {"shortDescription": [{"value": "Sphera Solutions GmbH", "lang": "en"}], "type": "contact data set", "refObjectId": "d7fa0337-f279-430d-becf-7f3111a85010", "version": "24.01.000", "uri": "../contacts/d7fa0337-f279-430d-becf-7f3111a85010.xml"}, "copyright": true, "licenseType": "Free of charge for all users and uses", "accessRestrictions": [{"value": "The license conditions as stated on https://www.oekobaudat.de/apply.", "lang": "en"}, {"value": "Es gelten die Lizenzbedingungen wie sie auf https://www.oekobaudat.de/ genannt sind.", "lang": "de"}], "other": {"anies": [{"name": "referenceToPublisher", "value": {"shortDescription": [{"value": "BBSR", "lang": "en"}], "type": "contact data set", "refObjectId": "f11651e0-7877-11e3-981f-0800200c9a66", "version": "00.01.000", "uri": "../contacts/f11651e0-7877-11e3-981f-0800200c9a66.xml"}}]}}}, "exchanges": {"exchange": [{"dataSetInternalID": 100551, "referenceToFlowDataSet": {"shortDescription": [{"value": "Insulated glazing, triple pane", "lang": "en"}, {"value": "Dreifachverglasung", "lang": "de"}], "type": "flow data set", "refObjectId": "472150d1-0e84-4dd5-98ba-18ee09bec971", "version": "24.01.000", "uri": "../flows/472150d1-0e84-4dd5-98ba-18ee09bec971.xml"}, "meanAmount": 1.0, "referenceFlow": true, "resultingflowAmount": 1.0, "flowProperties": [{"name": [{"lang": "en", "value": "Area"}, {"lang": "de", "value": "Fläche"}], "uuid": "93a60a56-a3c8-19da-a746-0800200c9a66", "referenceFlowProperty": true, "meanValue": 1.0, "referenceUnit": "qm", "unitGroupUUID": "c20a03d7-bd90-4569-bc94-66cfd364dfc8"}, {"name": [{"lang": "de", "value": "Masse"}, {"lang": "en", "value": "Mass"}], "uuid": "93a60a56-a3c8-11da-a746-0800200b9a66", "meanValue": 30.0}], "materialProperties": [{"name": "grammage", "value": "30.0", "unit": "kg/m^2", "unitDescription": "kilograms per square meter"}], "typeOfFlow": "Product flow", "classification": {"classHierarchy": "Valuable substances / Systems / Assemblies / Building industry", "name": "GaBiCategories"}}, {"dataSetInternalID": 100552, "referenceToFlowDataSet": {"shortDescription": [{"value": "Use of renewable primary energy as energy carrier (PERE)", "lang": "en"}, {"value": "Erneuerbare Primärenergie als Energieträger (PERE)", "lang": "de"}], "type": "flow data set", "refObjectId": "20f32be5-0398-4288-9b6d-accddd195317", "version": "24.01.000", "uri": "../flows/20f32be5-0398-4288-9b6d-accddd195317.xml"}, "exchange direction": "INPUT", "other": {"anies": [{"value": "91.4051957686329", "module": "A1-A3"}, {"name": "referenceToUnitGroupDataSet", "value": {"shortDescription": [{"value": "MJ", "lang": "en"}], "type": "unit group data set", "refObjectId": "93a60a57-a3c8-11da-a746-0800200c9a66", "version": "03.00.000", "uri": "../unitgroups/93a60a57-a3c8-11da-a746-0800200c9a66.xml"}}, {"value": "0.204323511248423", "module": "C2"}, {"value": "0.562886418957168", "module": "C3"}, {"value": "1.24401276240029", "module": "C4"}, {"value": "-5.79823001489368", "module": "D"}]}, "resolvedFlowVersion": "38.00.000", "flowProperties": [], "typeOfFlow": "Other flow", "classification": {"classHierarchy": "Quantities", "name": "GaBiCategories"}}, {"dataSetInternalID": 100553, "referenceToFlowDataSet": {"shortDescription": [{"value": "Use of renewable primary energy resources used as raw materials (PERM)", "lang": "en"}, {"value": "Erneuerbare Primärenergie zur stofflichen Nutzung (PERM)", "lang": "de"}], "type": "flow data set", "refObjectId": "fb3ec0de-548d-4508-aea5-00b73bf6f702", "version": "24.01.000", "uri": "../flows/fb3ec0de-548d-4508-aea5-00b73bf6f702.xml"}, "exchange direction": "INPUT", "other": {"anies": [{"value": "0", "module": "A1-A3"}, {"name": "referenceToUnitGroupDataSet", "value": {"shortDescription": [{"value": "MJ", "lang": "en"}], "type": "unit group data set", "refObjectId": "93a60a57-a3c8-11da-a746-0800200c9a66", "version": "03.00.000", "uri": "../unitgroups/93a60a57-a3c8-11da-a746-0800200c9a66.xml"}}, {"value": "0", "module": "C2"}, {"value": "0", "module": "C3"}, {"value": "0", "module": "C4"}, {"value": "0", "module": "D"}]}, "resolvedFlowVersion": "38.00.000", "flowProperties": [], "typeOfFlow": "Other flow", "classification": {"classHierarchy": "Quantities", "name": "GaBiCategories"}}, {"dataSetInternalID": 100554, "referenceToFlowDataSet": {"shortDescription": [{"value": "Total use of renewable primary energy (PERT)", "lang": "en"}, {"value": "Total erneuerbare Primärenergie (PERT)", "lang": "de"}], "type": "flow data set", "refObjectId": "53f97275-fa8a-4cdd-9024-65936002acd0", "version": "24.01.000", "uri": "../flows/53f97275-fa8a-4cdd-9024-65936002acd0.xml"}, "exchange direction": "INPUT", "other": {"anies": [{"value": "91.4051957686329", "module": "A1-A3"}, {"name": "referenceToUnitGroupDataSet", "value": {"shortDescription": [{"value": "MJ", "lang": "en"}], "type": "unit group data set", "refObjectId": "93a60a57-a3c8-11da-a746-0800200c9a66", "version": "03.00.000", "uri": "../unitgroups/93a60a57-a3c8-11da-a746-0800200c9a66.xml"}}, {"value": "0.204323511248423", "module": "C2"}, {"value": "0.562886418957168", "module": "C3"}, {"value": "1.24401276240029", "module": "C4"}, {"value": "-5.79823001489368", "module": "D"}]}, "resolvedFlowVersion": "38.00.000", "flowProperties": [], "typeOfFlow": "Other flow", "classification": {"classHierarchy": "Quantities / Environmental quantities / EPD EN 15804 / LCI indicators", "name": "GaBiCategories"}}, {"dataSetInternalID": 100555, "referenceToFlowDataSet": {"shortDescription": [{"value": "Use of non renewable primary energy as energy carrier (PENRE)", "lang": "en"}, {"value": "Nicht-erneuerbare Primärenergie als Energieträger (PENRE)", "lang": "de"}], "type": "flow data set", "refObjectId": "ac857178-2b45-46ec-892a-a9a4332f0372", "version": "24.01.000", "uri": "../flows/ac857178-2b45-46ec-892a-a9a4332f0372.xml"}, "exchange direction": "INPUT", "other": {"anies": [{"value": "673.82574876491", "module": "A1-A3"}, {"name": "referenceToUnitGroupDataSet", "value": {"shortDescription": [{"value": "MJ", "lang": "en"}], "type": "unit group data set", "refObjectId": "93a60a57-a3c8-11da-a746-0800200c9a66", "version": "03.00.000", "uri": "../unitgroups/93a60a57-a3c8-11da-a746-0800200c9a66.xml"}}, {"value": "1.84628302565341", "module": "C2"}, {"value": "44.7234862549151", "module": "C3"}, {"value": "7.10444012654796", "module": "C4"}, {"value": "-13.2640095383134", "module": "D"}]}, "resolvedFlowVersion": "38.00.000", "flowProperties": [], "typeOfFlow": "Other flow", "classification": {"classHierarchy": "Quantities", "name": "GaBiCategories"}}, {"dataSetInternalID": 100556, "referenceToFlowDataSet": {"shortDescription": [{"value": "Use of non renewable primary energy resources used as raw materials (PENRM)", "lang": "en"}, {"value": "Nicht-erneuerbare Primärenergie zur stofflichen Nutzung (PENRM)", "lang": "de"}], "type": "flow data set", "refObjectId": "1421caa0-679d-4bf4-b282-0eb850ccae27", "version": "24.01.000", "uri": "../flows/1421caa0-679d-4bf4-b282-0eb850ccae27.xml"}, "exchange direction": "INPUT", "other": {"anies": [{"value": "36", "module": "A1-A3"}, {"name": "referenceToUnitGroupDataSet", "value": {"shortDescription": [{"value": "MJ", "lang": "en"}], "type": "unit group data set", "refObjectId": "93a60a57-a3c8-11da-a746-0800200c9a66", "version": "03.00.000", "uri": "../unitgroups/93a60a57-a3c8-11da-a746-0800200c9a66.xml"}}, {"value": "0", "module": "C2"}, {"value": "-36", "module": "C3"}, {"value": "0", "module": "C4"}, {"value": "0", "module": "D"}]}, "resolvedFlowVersion": "38.00.000", "flowProperties": [], "typeOfFlow": "Other flow", "classification": {"classHierarchy": "Quantities", "name": "GaBiCategories"}}, {"dataSetInternalID": 100557, "referenceToFlowDataSet": {"shortDescription": [{"value": "Total use of non renewable primary energy resource (PENRT)", "lang": "en"}, {"value": "Total nicht-erneuerbare Primärenergie (PENRT)", "lang": "de"}], "type": "flow data set", "refObjectId": "06159210-646b-4c8d-8583-da9b3b95a6c1", "version": "24.01.000", "uri": "../flows/06159210-646b-4c8d-8583-da9b3b95a6c1.xml"}, "exchange direction": "INPUT", "other": {"anies": [{"value": "709.82574876491", "module": "A1-A3"}, {"name": "referenceToUnitGroupDataSet", "value": {"shortDescription": [{"value": "MJ", "lang": "en"}], "type": "unit group data set", "refObjectId": "93a60a57-a3c8-11da-a746-0800200c9a66", "version": "03.00.000", "uri": "../unitgroups/93a60a57-a3c8-11da-a746-0800200c9a66.xml"}}, {"value": "1.84628302565341", "module": "C2"}, {"value": "8.72348625491512", "module": "C3"}, {"value": "7.10444012654796", "module": "C4"}, {"value": "-13.2640095383134", "module": "D"}]}, "resolvedFlowVersion": "38.00.000", "flowProperties": [], "typeOfFlow": "Other flow", "classification": {"classHierarchy": "Quantities / Environmental quantities / EPD EN 15804 / LCI indicators", "name": "GaBiCategories"}}, {"dataSetInternalID": 100558, "referenceToFlowDataSet": {"shortDescription": [{"value": "Use of secondary material (SM)", "lang": "en"}, {"value": "Einsatz von Sekundärstoffen (SM)", "lang": "de"}], "type": "flow data set", "refObjectId": "c6a1f35f-2d09-4f54-8dfb-97e502e1ce92", "version": "24.01.000", "uri": "../flows/c6a1f35f-2d09-4f54-8dfb-97e502e1ce92.xml"}, "exchange direction": "INPUT", "other": {"anies": [{"value": "0", "module": "A1-A3"}, {"name": "referenceToUnitGroupDataSet", "value": {"shortDescription": [{"value": "kg", "lang": "en"}], "type": "unit group data set", "refObjectId": "93a60a57-a4c8-11da-a746-0800200c9a66", "version": "03.00.000", "uri": "../unitgroups/93a60a57-a4c8-11da-a746-0800200c9a66.xml"}}, {"value": "0", "module": "C2"}, {"value": "0", "module": "C3"}, {"value": "0", "module": "C4"}, {"value": "0", "module": "D"}]}, "resolvedFlowVersion": "38.00.000", "flowProperties": [], "typeOfFlow": "Other flow", "classification": {"classHierarchy": "Quantities / Environmental quantities / EPD EN 15804 / LCI indicators", "name": "GaBiCategories"}}, {"dataSetInternalID": 100559, "referenceToFlowDataSet": {"shortDescription": [{"value": "Use of renewable secondary fuels (SF)", "lang": "en"}, {"value": "Erneuerbare Sekundärbrennstoffe (SF)", "lang": "de"}], "type": "flow data set", "refObjectId": "64333088-a55f-4aa2-9a31-c10b07816787", "version": "24.01.000", "uri": "../flows/64333088-a55f-4aa2-9a31-c10b07816787.xml"}, "exchange direction": "INPUT", "other": {"anies": [{"value": "0", "module": "A1-A3"}, {"name": "referenceToUnitGroupDataSet", "value": {"shortDescription": [{"value": "MJ", "lang": "en"}], "type": "unit group data set", "refObjectId": "93a60a57-a3c8-11da-a746-0800200c9a66", "version": "03.00.000", "uri": "../unitgroups/93a60a57-a3c8-11da-a746-0800200c9a66.xml"}}, {"value": "0", "module": "C2"}, {"value": "0", "module": "C3"}, {"value": "0", "module": "C4"}, {"value": "0", "module": "D"}]}, "resolvedFlowVersion": "38.00.000", "flowProperties": [], "typeOfFlow": "Other flow", "classification": {"classHierarchy": "Quantities / Environmental quantities / EPD EN 15804 / LCI indicators", "name": "GaBiCategories"}}, {"dataSetInternalID": 100560, "referenceToFlowDataSet": {"shortDescription": [{"value": "Use of non renewable secondary fuels (NRSF)", "lang": "en"}, {"value": "Nicht erneuerbare Sekundärbrennstoffe (NRSF)", "lang": "de"}], "type": "flow data set", "refObjectId": "89def144-d39a-4287-b86f-efde453ddcb2", "version": "24.01.000", "uri": "../flows/89def144-d39a-4287-b86f-efde453ddcb2.xml"}, "exchange direction": "INPUT", "other": {"anies": [{"value": "0", "module": "A1-A3"}, {"name": "referenceToUnitGroupDataSet", "value": {"shortDescription": [{"value": "MJ", "lang": "en"}], "type": "unit group data set", "refObjectId": "93a60a57-a3c8-11da-a746-0800200c9a66", "version": "03.00.000", "uri": "../unitgroups/93a60a57-a3c8-11da-a746-0800200c9a66.xml"}}, {"value": "0", "module": "C2"}, {"value": "0", "module": "C3"}, {"value": "0", "module": "C4"}, {"value": "0", "module": "D"}]}, "resolvedFlowVersion": "38.00.000", "flowProperties": [], "typeOfFlow": "Other flow", "classification": {"classHierarchy": "Quantities / Environmental quantities / EPD EN 15804 / LCI indicators", "name": "GaBiCategories"}}, {"dataSetInternalID": 100561, "referenceToFlowDataSet": {"shortDescription": [{"value": "Net use of fresh water (FW)", "lang": "en"}, {"value": "Nettoeinsatz von Süßwasserressourcen (FW)", "lang": "de"}], "type": "flow data set", "refObjectId": "3cf952c8-f3a4-461d-8c96-96456ca62246", "version": "24.01.000", "uri": "../flows/3cf952c8-f3a4-461d-8c96-96456ca62246.xml"}, "exchange direction": "INPUT", "other": {"anies": [{"value": "0.119621714639294", "module": "A1-A3"}, {"name": "referenceToUnitGroupDataSet", "value": {"shortDescription": [{"value": "m3", "lang": "en"}], "type": "unit group data set", "refObjectId": "93a60a57-a3c8-12da-a746-0800200c9a66", "version": "03.00.000", "uri": "../unitgroups/93a60a57-a3c8-12da-a746-0800200c9a66.xml"}}, {"value": "0.000190882303474529", "module": "C2"}, {"value": "0.00680135349552901", "module": "C3"}, {"value": "0.00187959807348768", "module": "C4"}, {"value": "-0.00177317387271558", "module": "D"}]}, "resolvedFlowVersion": "38.00.000", "flowProperties": [], "typeOfFlow": "Other flow", "classification": {"classHierarchy": "Quantities / Environmental quantities / EPD EN 15804 / LCI indicators", "name": "GaBiCategories"}}, {"dataSetInternalID": 100562, "referenceToFlowDataSet": {"shortDescription": [{"value": "Hazardous waste disposed (HWD)", "lang": "en"}, {"value": "Gefährlicher Abfall zur Deponie (HWD)", "lang": "de"}], "type": "flow data set", "refObjectId": "430f9e0f-59b2-46a0-8e0d-55e0e84948fc", "version": "24.01.000", "uri": "../flows/430f9e0f-59b2-46a0-8e0d-55e0e84948fc.xml"}, "exchange direction": "OUTPUT", "other": {"anies": [{"value": "1.9408079457048E-7", "module": "A1-A3"}, {"name": "referenceToUnitGroupDataSet", "value": {"shortDescription": [{"value": "kg", "lang": "en"}], "type": "unit group data set", "refObjectId": "93a60a57-a4c8-11da-a746-0800200c9a66", "version": "03.00.000", "uri": "../unitgroups/93a60a57-a4c8-11da-a746-0800200c9a66.xml"}}, {"value": "8.98846334662682E-11", "module": "C2"}, {"value": "1.27051408160693E-9", "module": "C3"}, {"value": "1.78293983755549E-9", "module": "C4"}, {"value": "-1.23675379217304E-8", "module": "D"}]}, "resolvedFlowVersion": "38.00.000", "flowProperties": [], "typeOfFlow": "Other flow", "classification": {"classHierarchy": "Quantities / Environmental quantities / EPD EN 15804 / LCI indicators", "name": "GaBiCategories"}}, {"dataSetInternalID": 100563, "referenceToFlowDataSet": {"shortDescription": [{"value": "Non harzardous waste disposed (NHWD)", "lang": "en"}, {"value": "Entsorgter nicht gefährlicher Abfall (NHWD)", "lang": "de"}], "type": "flow data set", "refObjectId": "b29ef66b-e286-4afa-949f-62f1a7b4d7fa", "version": "24.01.000", "uri": "../flows/b29ef66b-e286-4afa-949f-62f1a7b4d7fa.xml"}, "exchange direction": "OUTPUT", "other": {"anies": [{"value": "3.67886635829215", "module": "A1-A3"}, {"name": "referenceToUnitGroupDataSet", "value": {"shortDescription": [{"value": "kg", "lang": "en"}], "type": "unit group data set", "refObjectId": "93a60a57-a4c8-11da-a746-0800200c9a66", "version": "03.00.000", "uri": "../unitgroups/93a60a57-a4c8-11da-a746-0800200c9a66.xml"}}, {"value": "0.000312164826977714", "module": "C2"}, {"value": "0.302819690795557", "module": "C3"}, {"value": "36.0344172898858", "module": "C4"}, {"value": "-0.00791528614555418", "module": "D"}]}, "resolvedFlowVersion": "38.00.000", "flowProperties": [], "typeOfFlow": "Other flow", "classification": {"classHierarchy": "Quantities / Environmental quantities / EPD EN 15804 / LCI indicators", "name": "GaBiCategories"}}, {"dataSetInternalID": 100564, "referenceToFlowDataSet": {"shortDescription": [{"value": "Radioactive waste disposed (RWD)", "lang": "en"}, {"value": "Entsorgter radioaktiver Abfall (RWD)", "lang": "de"}], "type": "flow data set", "refObjectId": "3449546e-52ad-4b39-b809-9fb77cea8ff6", "version": "24.01.000", "uri": "../flows/3449546e-52ad-4b39-b809-9fb77cea8ff6.xml"}, "exchange direction": "OUTPUT", "other": {"anies": [{"value": "0.00546379895578488", "module": "A1-A3"}, {"name": "referenceToUnitGroupDataSet", "value": {"shortDescription": [{"value": "kg", "lang": "en"}], "type": "unit group data set", "refObjectId": "93a60a57-a4c8-11da-a746-0800200c9a66", "version": "03.00.000", "uri": "../unitgroups/93a60a57-a4c8-11da-a746-0800200c9a66.xml"}}, {"value": "2.93867010283341E-6", "module": "C2"}, {"value": "4.850438390475E-5", "module": "C3"}, {"value": "7.35014372764389E-5", "module": "C4"}, {"value": "-0.000313727688884567", "module": "D"}]}, "resolvedFlowVersion": "38.00.000", "flowProperties": [], "typeOfFlow": "Other flow", "classification": {"classHierarchy": "Quantities / Environmental quantities / EPD EN 15804 / LCI indicators", "name": "GaBiCategories"}}, {"dataSetInternalID": 100565, "referenceToFlowDataSet": {"shortDescription": [{"value": "Components for re-use (CRU)", "lang": "en"}, {"value": "Komponenten für die Wiederverwendung (CRU)", "lang": "de"}], "type": "flow data set", "refObjectId": "a2b32f97-3fc7-4af2-b209-525bc6426f33", "version": "24.01.000", "uri": "../flows/a2b32f97-3fc7-4af2-b209-525bc6426f33.xml"}, "exchange direction": "OUTPUT", "other": {"anies": [{"value": "0", "module": "A1-A3"}, {"name": "referenceToUnitGroupDataSet", "value": {"shortDescription": [{"value": "kg", "lang": "en"}], "type": "unit group data set", "refObjectId": "93a60a57-a4c8-11da-a746-0800200c9a66", "version": "03.00.000", "uri": "../unitgroups/93a60a57-a4c8-11da-a746-0800200c9a66.xml"}}, {"value": "0", "module": "C2"}, {"value": "0", "module": "C3"}, {"value": "0", "module": "C4"}, {"value": "0", "module": "D"}]}, "resolvedFlowVersion": "38.00.000", "flowProperties": [], "typeOfFlow": "Other flow", "classification": {"classHierarchy": "Quantities / Environmental quantities / EPD EN 15804 / LCI indicators", "name": "GaBiCategories"}}, {"dataSetInternalID": 100566, "referenceToFlowDataSet": {"shortDescription": [{"value": "Materials for recycling  (MFR)", "lang": "en"}, {"value": "Stoffe zum Recycling (MFR)", "lang": "de"}], "type": "flow data set", "refObjectId": "d7fe48a5-4103-49c8-9aae-b0b5dfdbd6ae", "version": "24.01.000", "uri": "../flows/d7fe48a5-4103-49c8-9aae-b0b5dfdbd6ae.xml"}, "exchange direction": "OUTPUT", "other": {"anies": [{"value": "0", "module": "A1-A3"}, {"name": "referenceToUnitGroupDataSet", "value": {"shortDescription": [{"value": "kg", "lang": "en"}], "type": "unit group data set", "refObjectId": "93a60a57-a4c8-11da-a746-0800200c9a66", "version": "03.00.000", "uri": "../unitgroups/93a60a57-a4c8-11da-a746-0800200c9a66.xml"}}, {"value": "0", "module": "C2"}, {"value": "0", "module": "C3"}, {"value": "0", "module": "C4"}, {"value": "0", "module": "D"}]}, "resolvedFlowVersion": "38.00.000", "flowProperties": [], "typeOfFlow": "Other flow", "classification": {"classHierarchy": "Quantities / Environmental quantities / EPD EN 15804 / LCI indicators", "name": "GaBiCategories"}}, {"dataSetInternalID": 100567, "referenceToFlowDataSet": {"shortDescription": [{"value": "Materials for energy recovery (MER)", "lang": "en"}, {"value": "Stoffe für die Energierückgewinnung (MER)", "lang": "de"}], "type": "flow data set", "refObjectId": "59a9181c-3aaf-46ee-8b13-2b3723b6e447", "version": "24.01.000", "uri": "../flows/59a9181c-3aaf-46ee-8b13-2b3723b6e447.xml"}, "exchange direction": "OUTPUT", "other": {"anies": [{"value": "0", "module": "A1-A3"}, {"name": "referenceToUnitGroupDataSet", "value": {"shortDescription": [{"value": "kg", "lang": "en"}], "type": "unit group data set", "refObjectId": "93a60a57-a4c8-11da-a746-0800200c9a66", "version": "03.00.000", "uri": "../unitgroups/93a60a57-a4c8-11da-a746-0800200c9a66.xml"}}, {"value": "0", "module": "C2"}, {"value": "0", "module": "C3"}, {"value": "0", "module": "C4"}, {"value": "0", "module": "D"}]}, "resolvedFlowVersion": "38.00.000", "flowProperties": [], "typeOfFlow": "Other flow", "classification": {"classHierarchy": "Quantities / Environmental quantities / EPD EN 15804 / LCI indicators", "name": "GaBiCategories"}}, {"dataSetInternalID": 100568, "referenceToFlowDataSet": {"shortDescription": [{"value": "Exported electrical energy (EEE)", "lang": "en"}, {"value": "Exportierte elektrische Energie (EEE)", "lang": "de"}], "type": "flow data set", "refObjectId": "4da0c987-2b76-40d6-9e9e-82a017aaaf29", "version": "24.01.000", "uri": "../flows/4da0c987-2b76-40d6-9e9e-82a017aaaf29.xml"}, "exchange direction": "OUTPUT", "other": {"anies": [{"value": "0", "module": "A1-A3"}, {"name": "referenceToUnitGroupDataSet", "value": {"shortDescription": [{"value": "MJ", "lang": "en"}], "type": "unit group data set", "refObjectId": "93a60a57-a3c8-11da-a746-0800200c9a66", "version": "03.00.000", "uri": "../unitgroups/93a60a57-a3c8-11da-a746-0800200c9a66.xml"}}, {"value": "0", "module": "C2"}, {"value": "3.85756679478822", "module": "C3"}, {"value": "0", "module": "C4"}, {"value": "0", "module": "D"}]}, "resolvedFlowVersion": "38.00.000", "flowProperties": [], "typeOfFlow": "Other flow", "classification": {"classHierarchy": "Quantities / Environmental quantities / EPD EN 15804 / LCI indicators", "name": "GaBiCategories"}}, {"dataSetInternalID": 100569, "referenceToFlowDataSet": {"shortDescription": [{"value": "Exported thermal energy (EET)", "lang": "en"}, {"value": "Exportierte thermische Energie (EET)", "lang": "de"}], "type": "flow data set", "refObjectId": "98daf38a-7a79-46d3-9a37-2b7bd0955810", "version": "24.01.000", "uri": "../flows/98daf38a-7a79-46d3-9a37-2b7bd0955810.xml"}, "exchange direction": "OUTPUT", "other": {"anies": [{"value": "0", "module": "A1-A3"}, {"name": "referenceToUnitGroupDataSet", "value": {"shortDescription": [{"value": "MJ", "lang": "en"}], "type": "unit group data set", "refObjectId": "93a60a57-a3c8-11da-a746-0800200c9a66", "version": "03.00.000", "uri": "../unitgroups/93a60a57-a3c8-11da-a746-0800200c9a66.xml"}}, {"value": "0", "module": "C2"}, {"value": "8.93787993737", "module": "C3"}, {"value": "0", "module": "C4"}, {"value": "0", "module": "D"}]}, "resolvedFlowVersion": "38.00.000", "flowProperties": [], "typeOfFlow": "Other flow", "classification": {"classHierarchy": "Quantities / Environmental quantities / EPD EN 15804 / LCI indicators", "name": "GaBiCategories"}}]}, "LCIAResults": {"LCIAResult": [{"referenceToLCIAMethodDataSet": {"shortDescription": [{"value": "Climate change", "lang": "en"}, {"value": "Globales Erwärmungspotenzial - total (GWP-total)", "lang": "de"}], "type": "LCIA method data set", "refObjectId": "a7ea142a-9749-11ed-a8fc-0242ac120002", "version": "24.01.000", "uri": "../lciamethods/a7ea142a-9749-11ed-a8fc-0242ac120002.xml"}, "other": {"anies": [{"value": "59.7649122529103", "module": "A1-A3"}, {"value": "0.144007578993229", "module": "C2"}, {"value": "3.03032240426051", "module": "C3"}, {"value": "0.543642112367202", "module": "C4"}, {"value": "-0.948776941366316", "module": "D"}, {"name": "referenceToUnitGroupDataSet", "value": {"shortDescription": [{"value": "kg CO2 eq.", "lang": "en"}], "type": "unit group data set", "refObjectId": "1ebf3012-d0db-4de2-aefd-ef30cedb0be1", "version": "25.00.000", "uri": "../unitgroups/1ebf3012-d0db-4de2-aefd-ef30cedb0be1.xml"}}]}}, {"referenceToLCIAMethodDataSet": {"shortDescription": [{"value": "Climate change-Fossil", "lang": "en"}, {"value": "Globales Erwärmungspotenzial - fossil (GWP-fossil)", "lang": "de"}], "type": "LCIA method data set", "refObjectId": "a7ea19c0-9749-11ed-a8fc-0242ac120002", "version": "24.01.000", "uri": "../lciamethods/a7ea19c0-9749-11ed-a8fc-0242ac120002.xml"}, "other": {"anies": [{"value": "59.5637261523346", "module": "A1-A3"}, {"value": "0.140632565445917", "module": "C2"}, {"value": "3.02960097835259", "module": "C3"}, {"value": "0.539106203565284", "module": "C4"}, {"value": "-0.941305715093883", "module": "D"}, {"name": "referenceToUnitGroupDataSet", "value": {"shortDescription": [{"value": "kg CO2 eq.", "lang": "en"}], "type": "unit group data set", "refObjectId": "1ebf3012-d0db-4de2-aefd-ef30cedb0be1", "version": "25.00.000", "uri": "../unitgroups/1ebf3012-d0db-4de2-aefd-ef30cedb0be1.xml"}}]}}, {"referenceToLCIAMethodDataSet": {"shortDescription": [{"value": "Climate change-Biogenic", "lang": "en"}, {"value": "Globales Erwärmungspotenzial - biogen (GWP-biogenic)", "lang": "de"}], "type": "LCIA method data set", "refObjectId": "a7ea186c-9749-11ed-a8fc-0242ac120002", "version": "24.01.000", "uri": "../lciamethods/a7ea186c-9749-11ed-a8fc-0242ac120002.xml"}, "other": {"anies": [{"value": "0.126049248329716", "module": "A1-A3"}, {"value": "0.000670408717765095", "module": "C2"}, {"value": "0.00052648437000365", "module": "C3"}, {"value": "0.00130236069673097", "module": "C4"}, {"value": "-0.00735547498048849", "module": "D"}, {"name": "referenceToUnitGroupDataSet", "value": {"shortDescription": [{"value": "kg CO2 eq.", "lang": "en"}], "type": "unit group data set", "refObjectId": "1ebf3012-d0db-4de2-aefd-ef30cedb0be1", "version": "25.00.000", "uri": "../unitgroups/1ebf3012-d0db-4de2-aefd-ef30cedb0be1.xml"}}]}}, {"referenceToLCIAMethodDataSet": {"shortDescription": [{"value": "Climate change-Land use and land use change", "lang": "en"}, {"value": "Globales Erwärmungspotenzial - luluc (GWP-luluc)", "lang": "de"}], "type": "LCIA method data set", "refObjectId": "a7ea1ae2-9749-11ed-a8fc-0242ac120002", "version": "24.01.000", "uri": "../lciamethods/a7ea1ae2-9749-11ed-a8fc-0242ac120002.xml"}, "other": {"anies": [{"value": "0.0751368522460606", "module": "A1-A3"}, {"value": "0.00270460482954614", "module": "C2"}, {"value": "0.000194941537917933", "module": "C3"}, {"value": "0.00323354810518742", "module": "C4"}, {"value": "-0.000115751291943886", "module": "D"}, {"name": "referenceToUnitGroupDataSet", "value": {"shortDescription": [{"value": "kg CO2 eq.", "lang": "en"}], "type": "unit group data set", "refObjectId": "1ebf3012-d0db-4de2-aefd-ef30cedb0be1", "version": "25.00.000", "uri": "../unitgroups/1ebf3012-d0db-4de2-aefd-ef30cedb0be1.xml"}}]}}, {"referenceToLCIAMethodDataSet": {"shortDescription": [{"value": "Depletion potenzial of the stratospheric ozone layer (ODP)", "lang": "en"}, {"value": "Abbaupotenzial der stratosphärischen Ozonschicht (ODP)", "lang": "de"}], "type": "LCIA method data set", "refObjectId": "b5c629d6-def3-11e6-bf01-fe55135034f3", "version": "24.01.000", "uri": "../lciamethods/b5c629d6-def3-11e6-bf01-fe55135034f3.xml"}, "other": {"anies": [{"value": "2.03294318759089E-10", "module": "A1-A3"}, {"value": "4.44028079349567E-14", "module": "C2"}, {"value": "1.15261982552451E-12", "module": "C3"}, {"value": "1.46885741700429E-12", "module": "C4"}, {"value": "-1.42748700196817E-11", "module": "D"}, {"name": "referenceToUnitGroupDataSet", "value": {"shortDescription": [{"value": "kg CFC-11 eq.", "lang": "en"}], "type": "unit group data set", "refObjectId": "d9e957c9-7309-4474-bf3a-7777df6c4e5b", "version": "25.00.000", "uri": "../unitgroups/d9e957c9-7309-4474-bf3a-7777df6c4e5b.xml"}}]}}, {"referenceToLCIAMethodDataSet": {"shortDescription": [{"value": "Acidifcation potential, Accumulated Exceedance (AP)", "lang": "en"}, {"value": "Versauerungspotenzial, kumulierte Überschreitung (AP)", "lang": "de"}], "type": "LCIA method data set", "refObjectId": "b5c611c6-def3-11e6-bf01-fe55135034f3", "version": "24.01.000", "uri": "../lciamethods/b5c611c6-def3-11e6-bf01-fe55135034f3.xml"}, "other": {"anies": [{"value": "0.310904171064457", "module": "A1-A3"}, {"value": "0.000185625582043446", "module": "C2"}, {"value": "0.000513674249719188", "module": "C3"}, {"value": "0.00382631244526389", "module": "C4"}, {"value": "-0.000937412183214147", "module": "D"}, {"name": "referenceToUnitGroupDataSet", "value": {"shortDescription": [{"value": "Mole of H+ eq.", "lang": "en"}], "type": "unit group data set", "refObjectId": "42e089ac-92bf-4bf2-8ca1-5fc40d18f2ed", "version": "00.01.000", "uri": "../unitgroups/42e089ac-92bf-4bf2-8ca1-5fc40d18f2ed.xml"}}]}}, {"referenceToLCIAMethodDataSet": {"shortDescription": [{"value": "Eutrophication, freshwater", "lang": "en"}, {"value": "Eutrophierungspotenzial - Süßwasser (EP-freshwater)", "lang": "de"}], "type": "LCIA method data set", "refObjectId": "b53ec18f-7377-4ad3-86eb-cc3f4f276b2b", "version": "24.01.000", "uri": "../lciamethods/b53ec18f-7377-4ad3-86eb-cc3f4f276b2b.xml"}, "other": {"anies": [{"value": "5.99489053766762E-5", "module": "A1-A3"}, {"value": "3.82914147409343E-7", "module": "C2"}, {"value": "2.63985975526257E-7", "module": "C3"}, {"value": "1.22812890401317E-6", "module": "C4"}, {"value": "-2.31682364572953E-6", "module": "D"}, {"name": "referenceToUnitGroupDataSet", "value": {"shortDescription": [{"value": "kg P eq.", "lang": "en"}], "type": "unit group data set", "refObjectId": "0429039d-a61d-4590-ba67-aa4a20a810a1", "version": "25.00.000", "uri": "../unitgroups/0429039d-a61d-4590-ba67-aa4a20a810a1.xml"}}]}}, {"referenceToLCIAMethodDataSet": {"shortDescription": [{"value": "Eutrophication marine", "lang": "en"}, {"value": "Eutrophierungspotenzial - Salzwasser (EP-marine)", "lang": "de"}], "type": "LCIA method data set", "refObjectId": "b5c619fa-def3-11e6-bf01-fe55135034f3", "version": "24.01.000", "uri": "../lciamethods/b5c619fa-def3-11e6-bf01-fe55135034f3.xml"}, "other": {"anies": [{"value": "0.114292508673667", "module": "A1-A3"}, {"value": "6.57661946058088E-5", "module": "C2"}, {"value": "0.000113635325805319", "module": "C3"}, {"value": "0.000985079982668907", "module": "C4"}, {"value": "-0.000328442815889383", "module": "D"}, {"name": "referenceToUnitGroupDataSet", "value": {"shortDescription": [{"value": "kg N eq.", "lang": "en"}], "type": "unit group data set", "refObjectId": "d05bb823-ecdf-4686-8c40-bf1d9257859f", "version": "00.00.003", "uri": "../unitgroups/d05bb823-ecdf-4686-8c40-bf1d9257859f.xml"}}]}}, {"referenceToLCIAMethodDataSet": {"shortDescription": [{"value": "Eutrophication, terrestrial", "lang": "en"}, {"value": "Eutrophierungspotenzial - Land (EP-terrestrial)", "lang": "de"}], "type": "LCIA method data set", "refObjectId": "b5c614d2-def3-11e6-bf01-fe55135034f3", "version": "24.01.000", "uri": "../lciamethods/b5c614d2-def3-11e6-bf01-fe55135034f3.xml"}, "other": {"anies": [{"value": "1.3591768345053", "module": "A1-A3"}, {"value": "0.000799087690071463", "module": "C2"}, {"value": "0.00237801750031592", "module": "C3"}, {"value": "0.0108472896517858", "module": "C4"}, {"value": "-0.00349274317448149", "module": "D"}, {"name": "referenceToUnitGroupDataSet", "value": {"shortDescription": [{"value": "Mole of N eq.", "lang": "en"}], "type": "unit group data set", "refObjectId": "71b4d617-0ec9-4d3f-b65e-e438940c2401", "version": "00.00.003", "uri": "../unitgroups/71b4d617-0ec9-4d3f-b65e-e438940c2401.xml"}}]}}, {"referenceToLCIAMethodDataSet": {"shortDescription": [{"value": "Photochemical Ozone Creation Potential  (POCP)", "lang": "en"}, {"value": "Bildungspotenzial für troposphärisches Ozon (POCP)", "lang": "de"}], "type": "LCIA method data set", "refObjectId": "b5c610fe-def3-11e6-bf01-fe55135034f3", "version": "24.01.000", "uri": "../lciamethods/b5c610fe-def3-11e6-bf01-fe55135034f3.xml"}, "other": {"anies": [{"value": "0.294093945494691", "module": "A1-A3"}, {"value": "0.000180210572219672", "module": "C2"}, {"value": "0.000316934032160953", "module": "C3"}, {"value": "0.00301440668152303", "module": "C4"}, {"value": "-0.000865701449005769", "module": "D"}, {"name": "referenceToUnitGroupDataSet", "value": {"shortDescription": [{"value": "kg NMVOC eq.", "lang": "en"}], "type": "unit group data set", "refObjectId": "d27c25f8-fbc1-44c6-b47b-4adbae4199c6", "version": "00.00.003", "uri": "../unitgroups/d27c25f8-fbc1-44c6-b47b-4adbae4199c6.xml"}}]}}, {"referenceToLCIAMethodDataSet": {"shortDescription": [{"value": "Resource use, minerals and metals", "lang": "en"}, {"value": "Potenzial für die Verknappung abiotischer Ressourcen  nicht fossile Ressourcen (ADPE)", "lang": "de"}], "type": "LCIA method data set", "refObjectId": "b2ad6494-c78d-11e6-9d9d-cec0c932ce01", "version": "24.01.000", "uri": "../lciamethods/b2ad6494-c78d-11e6-9d9d-cec0c932ce01.xml"}, "other": {"anies": [{"value": "0.000222263116238728", "module": "A1-A3"}, {"value": "2.38620772231805E-8", "module": "C2"}, {"value": "9.90481934347598E-9", "module": "C3"}, {"value": "3.44516376218385E-8", "module": "C4"}, {"value": "-8.80686402386131E-8", "module": "D"}, {"name": "referenceToUnitGroupDataSet", "value": {"shortDescription": [{"value": "kg Sb eq.", "lang": "en"}], "type": "unit group data set", "refObjectId": "54ccd2d9-a32a-4fc2-923d-f2c8c93e89d4", "version": "25.00.000", "uri": "../unitgroups/54ccd2d9-a32a-4fc2-923d-f2c8c93e89d4.xml"}}]}}, {"referenceToLCIAMethodDataSet": {"shortDescription": [{"value": "Resource use, fossils", "lang": "en"}, {"value": "Potenzial für die Verknappung abiotischer Ressourcen  fossile Brennstoffe (ADPF)", "lang": "de"}], "type": "LCIA method data set", "refObjectId": "b2ad6110-c78d-11e6-9d9d-cec0c932ce01", "version": "24.01.000", "uri": "../lciamethods/b2ad6110-c78d-11e6-9d9d-cec0c932ce01.xml"}, "other": {"anies": [{"value": "717.019632832368", "module": "A1-A3"}, {"value": "1.84625122230736", "module": "C2"}, {"value": "1.5234714055935", "module": "C3"}, {"value": "7.10435115336566", "module": "C4"}, {"value": "-13.2638576887496", "module": "D"}, {"name": "referenceToUnitGroupDataSet", "value": {"shortDescription": [{"value": "MJ", "lang": "en"}], "type": "unit group data set", "refObjectId": "93a60a57-a3c8-11da-a746-0800200c9a66", "version": "02.00.000", "uri": "../unitgroups/93a60a57-a3c8-11da-a746-0800200c9a66.xml"}}]}}, {"referenceToLCIAMethodDataSet": {"shortDescription": [{"value": "Water use", "lang": "en"}, {"value": "Wasser-Entzugspotenzial (Benutzer) (WDP)", "lang": "de"}], "type": "LCIA method data set", "refObjectId": "b2ad66ce-c78d-11e6-9d9d-cec0c932ce01", "version": "24.01.000", "uri": "../lciamethods/b2ad66ce-c78d-11e6-9d9d-cec0c932ce01.xml"}, "other": {"anies": [{"value": "0.4925707429544", "module": "A1-A3"}, {"value": "0.00100783897809908", "module": "C2"}, {"value": "0.283516214910305", "module": "C3"}, {"value": "0.061504268631928", "module": "C4"}, {"value": "-0.0122519738608174", "module": "D"}, {"name": "referenceToUnitGroupDataSet", "value": {"shortDescription": [{"value": "m³ world equiv.", "lang": "en"}], "type": "unit group data set", "refObjectId": "6ae2df01-888e-46c8-b17d-49fa3869b476", "version": "00.00.003", "uri": "../unitgroups/6ae2df01-888e-46c8-b17d-49fa3869b476.xml"}}]}}]}, "otherAttributes": {"{http://www.indata.network/EPD/2019}epd-version": "1.2"}, "version": "1.1", "locations": "../ILCDLocations.xml"}