{"processInformation": {"dataSetInformation": {"UUID": "bce411da-4a65-4d3a-93b6-d91ed7560a4e", "name": {"baseName": [{"value": "Precast concrete elements for walls, pillars and beams Based on the concrete recipe Type 66b", "lang": "en"}]}, "classificationInformation": {"classification": [{"class": [{"value": "Mineralische Baustoffe", "level": 0, "classId": "1"}, {"value": "Steine und Elemente", "level": 1, "classId": "1.3"}, {"value": "Betonfertigteile und Betonwaren", "level": 2, "classId": "1.3.05"}], "name": "OEKOBAU.DAT"}]}, "generalComment": [{"value": "The average EPD (type: Cradle to gate with modules C1–C4 and module D) is about custom made precast concrete based on the concrete recipe type 66b, manufactured in Hattersheim, Germany. The calculation is based on 1 m³ of concrete with a share of 6 m% reinforcing and prestressed steel. Kiwa-Ecobility Experts shall not be liable with respect to manufacturer information, life cycle assessment data and evidences.", "lang": "en"}], "other": {"anies": [{"scenario": [{"description": [{"value": "The average proportion of prestressing steel at the Hattersheim site (type 66b) is 27,7 kg of steel. Modules B1 to B7: For concrete components, maintenance and repair measures are generally not necessary during the reference service life, so that no environmental burdens arise in these modules. In addition, no energy or water is consumed. C1 Demolition: According to the current state of the art, the demolition of concrete and reinforced concrete structures is mainly carried out with longfront excavators equipped with demolition clamps. The concrete buildings are demolished by so-called \"press cutting\", i.e. the crushing of concrete by applying a compressive force. It is estimated that one site vehicle is in operation for 30 minutes per sqm of concrete element (conservative assumption). C2 - C4 and D: It is assumed that concrete and reinforcement material are separated after deconstruction. For both waste groups, a waste scenario according to the Dutch National Environmental Database (NMD) (SBK 2019) is applied: Concrete (i.a. elements, brickwork): 99% of concrete is recycled and reused as aggregate.; Steel, reinforcement: 95% of reinforcing steel is marketed as scrap metal."}], "name": "Standard scenario", "default": true}]}]}}, "quantitativeReference": {"referenceToReferenceFlow": [1], "type": "Reference flow(s)"}, "time": {"referenceYear": 2020, "dataSetValidUntil": 2026, "timeRepresentativenessDescription": [{"value": "The reference year is 2020. All process-specific data was collected for the operating year 2020. The quantities of raw and auxiliary materials as well as energy consumption have been recorded and averaged over the entire operating year 2020.", "lang": "en"}], "other": {"anies": [{"name": "publicationDateOfEPD", "value": 1639699200000}]}}, "geography": {"locationOfOperationSupplyOrProduction": {"descriptionOfRestrictions": [{"value": "The geographical reference area is Germany.\r", "lang": "en"}], "location": "DE"}}, "technology": {"technologyDescriptionAndIncludedProcesses": [{"value": "The products are reinforced and prestressed precast concrete elements in various formats, sizes and applications. The elements are used as columns, walls and beams. The concrete type 66b has compressive strength class of C 55/67. The manufacturing contains the following processes: Delivery of raw materials; Preparation of the moulds (formwork, cutting and laying of the probation steel elements, placeholders); Concrete mixing and filling into the mould, curing; Removal of the formwork, finishing, storage.", "lang": "en"}], "technologicalApplicability": [{"value": "The products are prefabricated elements for building, civil engineering and bridge construction, balconies, solid ceilings.", "lang": "en"}], "referenceToTechnologyFlowDiagrammOrPicture": [{"shortDescription": [{"value": "Flow chart Precast concrete elements for walls, pillars and beams Based on the concrete recipe Type 66b", "lang": "en"}], "type": "source data set", "refObjectId": "b419d8b6-d7db-4153-ac5f-39b5f99bab5c", "version": "00.00.002"}]}}, "modellingAndValidation": {"LCIMethodAndAllocation": {"typeOfDataSet": "EPD", "other": {"anies": [{"name": "subType", "value": "average dataset"}]}}, "dataSourcesTreatmentAndRepresentativeness": {"referenceToDataSource": [{"shortDescription": [{"value": "ecoinvent 3.6 database", "lang": "en"}], "type": "source data set", "refObjectId": "766b9973-5ee8-48a2-8098-72c8e20b369f", "version": "00.00.001"}, {"shortDescription": [{"value": "ecoinvent database (general)", "lang": "en"}], "type": "source data set", "refObjectId": "b497a91f-e14b-4b69-8f28-f50eb1576766", "version": "00.03.002"}], "useAdviceForDataSet": [{"value": "The products are prefabricated elements for building, civil engineering and bridge construction, balconies, solid ceilings.", "lang": "en"}], "other": {"anies": [{"name": "referenceToOriginalEPD", "value": {"shortDescription": {"value": "Precast concrete elements for walls, pillars and beams Based on the concrete recipe Type 66b EPD", "defaultValue": "Precast concrete elements for walls, pillars and beams Based on the concrete recipe Type 66b EPD", "lstrings": [{"lang": "en", "value": "Precast concrete elements for walls, pillars and beams Based on the concrete recipe Type 66b EPD"}]}, "version": {"version": 1, "majorVersion": 0, "minorVersion": 0, "subMinorVersion": 1, "zero": false, "versionString": "00.00.001"}, "type": "source data set", "uuid": {"uuid": "6fd61f91-eedf-4a21-b4e1-72731c8dec53"}, "refObjectId": "6fd61f91-eedf-4a21-b4e1-72731c8dec53", "versionAsString": "00.00.001", "resourceURLs": ["https://oekobaudat.de/OEKOBAU.DAT/resource/sources/6fd61f91-eedf-4a21-b4e1-72731c8dec53/EPD-Holcon-160-EN (Rev.1_26.04.2023).pdf?version=00.00.001"]}}]}}, "validation": {"review": [{"reviewDetails": [{"value": "An independent verification of the declaration and data according to ISO 14025:2011-10\r has been performed.", "lang": "en"}], "referenceToNameOfReviewerAndInstitution": [{"shortDescription": [{"value": "Max Sonnen (External verifier – Ecomatters)", "lang": "en"}], "type": "contact data set", "refObjectId": "be3e97ec-7946-4c02-a785-3e22ff35d8ad", "version": "00.00.001"}], "type": "Independent external review"}]}, "complianceDeclarations": {"compliance": [{"referenceToComplianceSystem": {"shortDescription": [{"value": "EN 15804+A2", "lang": "de"}, {"value": "EN 15804+A2", "lang": "en"}], "type": "source data set", "refObjectId": "c0016b33-8cf7-415c-ac6e-deba0d21440d", "version": "00.01.000"}}, {"referenceToComplianceSystem": {"shortDescription": [{"value": "ISO 14025", "lang": "en"}], "type": "source data set", "refObjectId": "4f2eb655-6e44-4874-a95a-e28f5442cd4d", "version": "00.00.001"}}]}}, "administrativeInformation": {"commissionerAndGoal": {"referenceToCommissioner": [{"shortDescription": [{"value": "Holcon GmbH", "lang": "en"}], "type": "contact data set", "refObjectId": "77887aab-4427-4387-869e-b593399859ae", "version": "00.00.001"}]}, "dataGenerator": {"referenceToPersonOrEntityGeneratingTheDataSet": [{"shortDescription": [{"value": "Kiwa GmbH (Berlin)", "lang": "en"}], "type": "contact data set", "refObjectId": "3ea4a87a-3f88-4633-b7e7-1bbdd272be43", "version": "00.00.001"}]}, "dataEntryBy": {"timeStamp": 1711541964001, "referenceToDataSetFormat": [{"shortDescription": [{"value": "EPD Data Format Extensions v1.2", "lang": "en"}, {"value": "EPD-Datenformaterweiterungen v1.2", "lang": "de"}], "type": "source data set", "refObjectId": "a29449fd-aa2f-4de8-b5d7-4b06b43c6fde", "version": "00.01.000"}, {"shortDescription": [{"value": "ILCD format", "lang": "en"}], "type": "source data set", "refObjectId": "a97a0155-0234-4b87-b4ce-a45da52f2a40", "version": "01.00.000", "uri": "http://lca.jrc.ec.europa.eu/lcainfohub/sample_data/ilcd/sources/ILCD_Format_a97a0155-0234-4b87-b4ce-a45da52f2a40_01.00.000.xml"}], "referenceToPersonOrEntityEnteringTheData": {"shortDescription": [{"value": "Kiwa GmbH (Berlin)", "lang": "en"}], "type": "contact data set", "refObjectId": "3ea4a87a-3f88-4633-b7e7-1bbdd272be43", "version": "00.00.001"}}, "publicationAndOwnership": {"dataSetVersion": "00.00.007", "referenceToRegistrationAuthority": {"shortDescription": [{"value": "Kiwa-Ecobility Experts, Kiwa GmbH (Berlin)", "lang": "en"}], "type": "contact data set", "refObjectId": "eb52a9a8-9d0f-40ce-a5c9-7b78f5615e5a", "version": "00.00.001"}, "registrationNumber": "EPD-Holcon-160-EN (Rev.1_26.04.2023)", "referenceToOwnershipOfDataSet": {"shortDescription": [{"value": "Holcon GmbH", "lang": "en"}], "type": "contact data set", "refObjectId": "77887aab-4427-4387-869e-b593399859ae", "version": "00.00.001"}, "copyright": true, "licenseType": "Free of charge for all users and uses", "accessRestrictions": [{"value": "None.", "lang": "en"}], "other": {"anies": [{"name": "referenceToPublisher", "value": {"shortDescription": [{"value": "Kiwa-Ecobility Experts, Kiwa GmbH (Berlin)", "lang": "en"}], "type": "contact data set", "refObjectId": "eb52a9a8-9d0f-40ce-a5c9-7b78f5615e5a", "version": "00.00.001"}}]}}}, "exchanges": {"exchange": [{"dataSetInternalID": 1, "referenceToFlowDataSet": {"shortDescription": [{"value": "Precast concrete elements for walls, pillars and beams Based on the concrete recipe Type 66b", "lang": "en"}], "type": "flow data set", "refObjectId": "89b6bfca-cdfb-4d2e-b973-63dbd126b0ea", "version": "00.00.001"}, "meanAmount": 1.0, "resultingAmount": 1.0, "referenceFlow": true, "resultingflowAmount": 1.0, "flowProperties": [{"name": [{"lang": "en", "value": "Volume"}, {"lang": "de", "value": "Volumen"}], "uuid": "93a60a56-a3c8-22da-a746-0800200c9a66", "referenceFlowProperty": true, "meanValue": 1.0, "referenceUnit": "m3", "unitGroupUUID": "cd950537-0a98-4044-9ba7-9f9a68d0a504"}], "materialProperties": [{"name": "gross density", "value": "2417.1", "unit": "kg/m^3", "unitDescription": "kilograms per cubic metre"}], "typeOfFlow": "Product flow", "classification": {"classHierarchy": "Mineralische Baustoffe / Steine und Elemente / Betonfertigteile und Betonwaren", "name": "OEKOBAU.DAT"}}, {"dataSetInternalID": 2, "referenceToFlowDataSet": {"shortDescription": [{"value": "Komponenten für die Wiederverwendung (CRU)", "lang": "de"}, {"value": "Components for re-use (CRU)", "lang": "en"}, {"value": "Componentes para su reutilización (CRU)", "lang": "es"}, {"value": "Komponenter för återanvändning (CRU)", "lang": "sv"}], "type": "flow data set", "refObjectId": "a2b32f97-3fc7-4af2-b209-525bc6426f33", "version": "30.00.002"}, "exchange direction": "OUTPUT", "meanAmount": 0.0, "other": {"anies": [{"value": "0.0", "module": "A1", "scenario": "Standard scenario"}, {"value": "0.0", "module": "A2", "scenario": "Standard scenario"}, {"value": "0.0", "module": "A3", "scenario": "Standard scenario"}, {"value": "0.0", "module": "C1", "scenario": "Standard scenario"}, {"value": "0.0", "module": "C2", "scenario": "Standard scenario"}, {"value": "0.0", "module": "C3", "scenario": "Standard scenario"}, {"value": "0.0", "module": "C4", "scenario": "Standard scenario"}, {"value": "0.0", "module": "D", "scenario": "Standard scenario"}, {"name": "referenceToUnitGroupDataSet", "value": {"shortDescription": [{"value": "kg"}], "type": "unit group data set", "refObjectId": "ad38d542-3fe9-439d-9b95-2f5f7752acaf", "uri": "../unitgroups/ad38d542-3fe9-439d-9b95-2f5f7752acaf"}}]}, "resolvedFlowVersion": "38.00.000", "flowProperties": [], "typeOfFlow": "Other flow", "classification": {"classHierarchy": "Quantities / Environmental quantities / EPD EN 15804 / LCI indicators", "name": "GaBiCategories"}}, {"dataSetInternalID": 3, "referenceToFlowDataSet": {"shortDescription": [{"value": "Exportierte elektrische Energie (EEE)", "lang": "de"}, {"value": "Exported electrical energy (EEE)", "lang": "en"}, {"value": "Energía exportada electrica (EEE)", "lang": "es"}, {"value": "Exporterad energi – elektrisk (EEE)", "lang": "sv"}], "type": "flow data set", "refObjectId": "4da0c987-2b76-40d6-9e9e-82a017aaaf29", "version": "30.00.002"}, "exchange direction": "OUTPUT", "meanAmount": 0.0, "other": {"anies": [{"value": "0.0", "module": "A1", "scenario": "Standard scenario"}, {"value": "0.0", "module": "A2", "scenario": "Standard scenario"}, {"value": "0.0471", "module": "A3", "scenario": "Standard scenario"}, {"value": "0.0", "module": "C1", "scenario": "Standard scenario"}, {"value": "0.0", "module": "C2", "scenario": "Standard scenario"}, {"value": "0.0", "module": "C3", "scenario": "Standard scenario"}, {"value": "0.0", "module": "C4", "scenario": "Standard scenario"}, {"value": "0.00141", "module": "D", "scenario": "Standard scenario"}, {"name": "referenceToUnitGroupDataSet", "value": {"shortDescription": [{"value": "MJ"}], "type": "unit group data set", "refObjectId": "93a60a57-a3c8-11da-a746-0800200c9a66", "uri": "../unitgroups/93a60a57-a3c8-11da-a746-0800200c9a66"}}]}, "resolvedFlowVersion": "38.00.000", "flowProperties": [], "typeOfFlow": "Other flow", "classification": {"classHierarchy": "Quantities / Environmental quantities / EPD EN 15804 / LCI indicators", "name": "GaBiCategories"}}, {"dataSetInternalID": 4, "referenceToFlowDataSet": {"shortDescription": [{"value": "Exportierte thermische Energie (EET)", "lang": "de"}, {"value": "Exported thermal energy (EET)", "lang": "en"}, {"value": "Energía exportada termal (EET)", "lang": "es"}, {"value": "Exporterad energi – termisk (EET)", "lang": "sv"}], "type": "flow data set", "refObjectId": "98daf38a-7a79-46d3-9a37-2b7bd0955810", "version": "30.00.002"}, "exchange direction": "OUTPUT", "meanAmount": 0.0, "other": {"anies": [{"value": "0.0", "module": "A1", "scenario": "Standard scenario"}, {"value": "0.0", "module": "A2", "scenario": "Standard scenario"}, {"value": "0.0811", "module": "A3", "scenario": "Standard scenario"}, {"value": "0.0", "module": "C1", "scenario": "Standard scenario"}, {"value": "0.0", "module": "C2", "scenario": "Standard scenario"}, {"value": "0.0", "module": "C3", "scenario": "Standard scenario"}, {"value": "0.0", "module": "C4", "scenario": "Standard scenario"}, {"value": "0.00243", "module": "D", "scenario": "Standard scenario"}, {"name": "referenceToUnitGroupDataSet", "value": {"shortDescription": [{"value": "MJ"}], "type": "unit group data set", "refObjectId": "93a60a57-a3c8-11da-a746-0800200c9a66", "uri": "../unitgroups/93a60a57-a3c8-11da-a746-0800200c9a66"}}]}, "resolvedFlowVersion": "38.00.000", "flowProperties": [], "typeOfFlow": "Other flow", "classification": {"classHierarchy": "Quantities / Environmental quantities / EPD EN 15804 / LCI indicators", "name": "GaBiCategories"}}, {"dataSetInternalID": 5, "referenceToFlowDataSet": {"shortDescription": [{"value": "Gefährlicher Abfall zur Deponie (HWD)", "lang": "de"}, {"value": "Hazardous waste disposed (HWD)", "lang": "en"}, {"value": "Residuos peligrosos eliminados (HWD)", "lang": "es"}, {"value": "Farligt avfall (HWD)", "lang": "sv"}], "type": "flow data set", "refObjectId": "430f9e0f-59b2-46a0-8e0d-55e0e84948fc", "version": "30.00.002"}, "exchange direction": "OUTPUT", "meanAmount": 0.0, "other": {"anies": [{"value": "0.0169", "module": "A1", "scenario": "Standard scenario"}, {"value": "0.00282", "module": "A2", "scenario": "Standard scenario"}, {"value": "0.00113", "module": "A3", "scenario": "Standard scenario"}, {"value": "0.00196", "module": "C1", "scenario": "Standard scenario"}, {"value": "0.00122", "module": "C2", "scenario": "Standard scenario"}, {"value": "1.8E-4", "module": "C3", "scenario": "Standard scenario"}, {"value": "1.27E-5", "module": "C4", "scenario": "Standard scenario"}, {"value": "-0.0094", "module": "D", "scenario": "Standard scenario"}, {"name": "referenceToUnitGroupDataSet", "value": {"shortDescription": [{"value": "kg"}], "type": "unit group data set", "refObjectId": "ad38d542-3fe9-439d-9b95-2f5f7752acaf", "uri": "../unitgroups/ad38d542-3fe9-439d-9b95-2f5f7752acaf"}}]}, "resolvedFlowVersion": "38.00.000", "flowProperties": [], "typeOfFlow": "Other flow", "classification": {"classHierarchy": "Quantities / Environmental quantities / EPD EN 15804 / LCI indicators", "name": "GaBiCategories"}}, {"dataSetInternalID": 6, "referenceToFlowDataSet": {"shortDescription": [{"value": "Stoffe für die Energierückgewinnung (MER)", "lang": "de"}, {"value": "Materials for energy recovery (MER)", "lang": "en"}, {"value": "Materiales para valorización energética (recuperación de energía) (MER)", "lang": "es"}, {"value": "Material till energiåtervinning (MER)", "lang": "sv"}], "type": "flow data set", "refObjectId": "59a9181c-3aaf-46ee-8b13-2b3723b6e447", "version": "30.00.002"}, "exchange direction": "OUTPUT", "meanAmount": 0.0, "other": {"anies": [{"value": "0.0", "module": "A1", "scenario": "Standard scenario"}, {"value": "0.0", "module": "A2", "scenario": "Standard scenario"}, {"value": "0.0", "module": "A3", "scenario": "Standard scenario"}, {"value": "0.0", "module": "C1", "scenario": "Standard scenario"}, {"value": "0.0", "module": "C2", "scenario": "Standard scenario"}, {"value": "0.0", "module": "C3", "scenario": "Standard scenario"}, {"value": "0.0", "module": "C4", "scenario": "Standard scenario"}, {"value": "0.0", "module": "D", "scenario": "Standard scenario"}, {"name": "referenceToUnitGroupDataSet", "value": {"shortDescription": [{"value": "kg"}], "type": "unit group data set", "refObjectId": "ad38d542-3fe9-439d-9b95-2f5f7752acaf", "uri": "../unitgroups/ad38d542-3fe9-439d-9b95-2f5f7752acaf"}}]}, "resolvedFlowVersion": "38.00.000", "flowProperties": [], "typeOfFlow": "Other flow", "classification": {"classHierarchy": "Quantities / Environmental quantities / EPD EN 15804 / LCI indicators", "name": "GaBiCategories"}}, {"dataSetInternalID": 7, "referenceToFlowDataSet": {"shortDescription": [{"value": "Stoffe zum Recycling (MFR)", "lang": "de"}, {"value": "Materials for recycling (MFR)", "lang": "en"}, {"value": "Materiales para el reciclaje (MFR)", "lang": "es"}, {"value": "Material till återvinning (MFR)", "lang": "sv"}], "type": "flow data set", "refObjectId": "d7fe48a5-4103-49c8-9aae-b0b5dfdbd6ae", "version": "30.00.002"}, "exchange direction": "OUTPUT", "meanAmount": 0.0, "other": {"anies": [{"value": "0.0", "module": "A1", "scenario": "Standard scenario"}, {"value": "0.0", "module": "A2", "scenario": "Standard scenario"}, {"value": "47.8", "module": "A3", "scenario": "Standard scenario"}, {"value": "0.0", "module": "C1", "scenario": "Standard scenario"}, {"value": "0.0", "module": "C2", "scenario": "Standard scenario"}, {"value": "4920.0", "module": "C3", "scenario": "Standard scenario"}, {"value": "0.0", "module": "C4", "scenario": "Standard scenario"}, {"value": "0.0", "module": "D", "scenario": "Standard scenario"}, {"name": "referenceToUnitGroupDataSet", "value": {"shortDescription": [{"value": "kg"}], "type": "unit group data set", "refObjectId": "ad38d542-3fe9-439d-9b95-2f5f7752acaf", "uri": "../unitgroups/ad38d542-3fe9-439d-9b95-2f5f7752acaf"}}]}, "resolvedFlowVersion": "38.00.000", "flowProperties": [], "typeOfFlow": "Other flow", "classification": {"classHierarchy": "Quantities / Environmental quantities / EPD EN 15804 / LCI indicators", "name": "GaBiCategories"}}, {"dataSetInternalID": 8, "referenceToFlowDataSet": {"shortDescription": [{"value": "Einsatz von Süßwasserressourcen (FW)", "lang": "de"}, {"value": "Use of net fresh water (FW)", "lang": "en"}, {"value": "Uso neto de recursos de agua dulce (FW)", "lang": "es"}, {"value": "Användning av sötvatten (FW)", "lang": "sv"}], "type": "flow data set", "refObjectId": "3cf952c8-f3a4-461d-8c96-96456ca62246", "version": "30.00.003"}, "exchange direction": "INPUT", "meanAmount": 0.0, "other": {"anies": [{"value": "10.1", "module": "A1", "scenario": "Standard scenario"}, {"value": "0.161", "module": "A2", "scenario": "Standard scenario"}, {"value": "0.437", "module": "A3", "scenario": "Standard scenario"}, {"value": "0.0371", "module": "C1", "scenario": "Standard scenario"}, {"value": "0.0585", "module": "C2", "scenario": "Standard scenario"}, {"value": "0.0345", "module": "C3", "scenario": "Standard scenario"}, {"value": "0.00909", "module": "C4", "scenario": "Standard scenario"}, {"value": "-7.15", "module": "D", "scenario": "Standard scenario"}, {"name": "referenceToUnitGroupDataSet", "value": {"shortDescription": [{"value": "m3"}], "type": "unit group data set", "refObjectId": "cd950537-0a98-4044-9ba7-9f9a68d0a504", "uri": "../unitgroups/cd950537-0a98-4044-9ba7-9f9a68d0a504"}}]}, "resolvedFlowVersion": "38.00.000", "flowProperties": [], "typeOfFlow": "Other flow", "classification": {"classHierarchy": "Quantities / Environmental quantities / EPD EN 15804 / LCI indicators", "name": "GaBiCategories"}}, {"dataSetInternalID": 9, "referenceToFlowDataSet": {"shortDescription": [{"value": "Entsorgter nicht gefährlicher Abfall (NHWD)", "lang": "de"}, {"value": "Non hazardous waste dispose (NHWD)", "lang": "en"}, {"value": "Residuos no peligrosos eliminados (NHWD)", "lang": "es"}, {"value": "Icke-farligt avfall (NHWD)", "lang": "sv"}], "type": "flow data set", "refObjectId": "b29ef66b-e286-4afa-949f-62f1a7b4d7fa", "version": "30.00.002"}, "exchange direction": "OUTPUT", "meanAmount": 0.0, "other": {"anies": [{"value": "81.3", "module": "A1", "scenario": "Standard scenario"}, {"value": "47.3", "module": "A2", "scenario": "Standard scenario"}, {"value": "5.63", "module": "A3", "scenario": "Standard scenario"}, {"value": "0.854", "module": "C1", "scenario": "Standard scenario"}, {"value": "30.4", "module": "C2", "scenario": "Standard scenario"}, {"value": "14.4", "module": "C3", "scenario": "Standard scenario"}, {"value": "57.8", "module": "C4", "scenario": "Standard scenario"}, {"value": "-10.5", "module": "D", "scenario": "Standard scenario"}, {"name": "referenceToUnitGroupDataSet", "value": {"shortDescription": [{"value": "kg"}], "type": "unit group data set", "refObjectId": "ad38d542-3fe9-439d-9b95-2f5f7752acaf", "uri": "../unitgroups/ad38d542-3fe9-439d-9b95-2f5f7752acaf"}}]}, "resolvedFlowVersion": "38.00.000", "flowProperties": [], "typeOfFlow": "Other flow", "classification": {"classHierarchy": "Quantities / Environmental quantities / EPD EN 15804 / LCI indicators", "name": "GaBiCategories"}}, {"dataSetInternalID": 10, "referenceToFlowDataSet": {"shortDescription": [{"value": "Nicht-erneuerbare Primärenergie als Energieträger (PENRE)", "lang": "de"}, {"value": "Use of non renewable primary energy (PENRE)", "lang": "en"}, {"value": "Uso de energía primaria no renovable, excluyendo los recursos de energía primaria no renovable utilizada como materia prima (PENRE)", "lang": "es"}, {"value": "Icke förnybar primärenergi - använd som energibärare (PENRE)", "lang": "sv"}], "type": "flow data set", "refObjectId": "ac857178-2b45-46ec-892a-a9a4332f0372", "version": "30.00.002"}, "exchange direction": "INPUT", "meanAmount": 0.0, "other": {"anies": [{"value": "6330.0", "module": "A1", "scenario": "Standard scenario"}, {"value": "1170.0", "module": "A2", "scenario": "Standard scenario"}, {"value": "1560.0", "module": "A3", "scenario": "Standard scenario"}, {"value": "766.0", "module": "C1", "scenario": "Standard scenario"}, {"value": "510.0", "module": "C2", "scenario": "Standard scenario"}, {"value": "110.0", "module": "C3", "scenario": "Standard scenario"}, {"value": "9.04", "module": "C4", "scenario": "Standard scenario"}, {"value": "-753.0", "module": "D", "scenario": "Standard scenario"}, {"name": "referenceToUnitGroupDataSet", "value": {"shortDescription": [{"value": "MJ"}], "type": "unit group data set", "refObjectId": "93a60a57-a3c8-11da-a746-0800200c9a66", "uri": "../unitgroups/93a60a57-a3c8-11da-a746-0800200c9a66"}}]}, "resolvedFlowVersion": "38.00.000", "flowProperties": [], "typeOfFlow": "Other flow", "classification": {"classHierarchy": "Quantities", "name": "GaBiCategories"}}, {"dataSetInternalID": 11, "referenceToFlowDataSet": {"shortDescription": [{"value": "Nicht-erneuerbare Primärenergie zur stofflichen Nutzung (PENRM)", "lang": "de"}, {"value": "Use of non renewable primary energy resources used as raw materials (PENRM)", "lang": "en"}, {"value": "Uso de la energía primaria no renovable utilizada como materia prima (PENRM)", "lang": "es"}, {"value": "Icke förnybar primärenergi - använd som råmaterial (PENRM)", "lang": "sv"}], "type": "flow data set", "refObjectId": "1421caa0-679d-4bf4-b282-0eb850ccae27", "version": "30.00.001"}, "exchange direction": "INPUT", "meanAmount": 0.0, "other": {"anies": [{"value": "0.0", "module": "A1", "scenario": "Standard scenario"}, {"value": "0.0", "module": "A2", "scenario": "Standard scenario"}, {"value": "0.0", "module": "A3", "scenario": "Standard scenario"}, {"value": "0.0", "module": "C1", "scenario": "Standard scenario"}, {"value": "0.0", "module": "C2", "scenario": "Standard scenario"}, {"value": "0.0", "module": "C3", "scenario": "Standard scenario"}, {"value": "0.0", "module": "C4", "scenario": "Standard scenario"}, {"value": "0.0", "module": "D", "scenario": "Standard scenario"}, {"name": "referenceToUnitGroupDataSet", "value": {"shortDescription": [{"value": "MJ"}], "type": "unit group data set", "refObjectId": "93a60a57-a3c8-11da-a746-0800200c9a66", "uri": "../unitgroups/93a60a57-a3c8-11da-a746-0800200c9a66"}}]}, "resolvedFlowVersion": "38.00.000", "flowProperties": [], "typeOfFlow": "Other flow", "classification": {"classHierarchy": "Quantities", "name": "GaBiCategories"}}, {"dataSetInternalID": 12, "referenceToFlowDataSet": {"shortDescription": [{"value": "Nicht erneuerbare Sekundärbrennstoffe (NRSF)", "lang": "de"}, {"value": "Use of non renewable secondary fuels (NRSF)", "lang": "en"}, {"value": "Uso de combustibles secundarios no renovables (NRSF)", "lang": "es"}, {"value": "Användning av ickeförnybara sekundära bränslen (NRSF)", "lang": "sv"}], "type": "flow data set", "refObjectId": "89def144-d39a-4287-b86f-efde453ddcb2", "version": "30.00.001"}, "exchange direction": "INPUT", "meanAmount": 0.0, "other": {"anies": [{"value": "0.0", "module": "A1", "scenario": "Standard scenario"}, {"value": "0.0", "module": "A2", "scenario": "Standard scenario"}, {"value": "0.0", "module": "A3", "scenario": "Standard scenario"}, {"value": "0.0", "module": "C1", "scenario": "Standard scenario"}, {"value": "0.0", "module": "C2", "scenario": "Standard scenario"}, {"value": "0.0", "module": "C3", "scenario": "Standard scenario"}, {"value": "0.0", "module": "C4", "scenario": "Standard scenario"}, {"value": "0.0", "module": "D", "scenario": "Standard scenario"}, {"name": "referenceToUnitGroupDataSet", "value": {"shortDescription": [{"value": "MJ"}], "type": "unit group data set", "refObjectId": "93a60a57-a3c8-11da-a746-0800200c9a66", "uri": "../unitgroups/93a60a57-a3c8-11da-a746-0800200c9a66"}}]}, "resolvedFlowVersion": "38.00.000", "flowProperties": [], "typeOfFlow": "Other flow", "classification": {"classHierarchy": "Quantities / Environmental quantities / EPD EN 15804 / LCI indicators", "name": "GaBiCategories"}}, {"dataSetInternalID": 13, "referenceToFlowDataSet": {"shortDescription": [{"value": "Entsorgter radioaktiver Abfall (RWD)", "lang": "de"}, {"value": "Radioactive waste disposed (RWD)", "lang": "en"}, {"value": "Residuos radiactivos eliminados (RWD)", "lang": "es"}, {"value": "Radioaktivt avfall (RWD) ", "lang": "sv"}], "type": "flow data set", "refObjectId": "3449546e-52ad-4b39-b809-9fb77cea8ff6", "version": "30.00.001"}, "exchange direction": "OUTPUT", "meanAmount": 0.0, "other": {"anies": [{"value": "0.0252", "module": "A1", "scenario": "Standard scenario"}, {"value": "0.0072", "module": "A2", "scenario": "Standard scenario"}, {"value": "0.00448", "module": "A3", "scenario": "Standard scenario"}, {"value": "0.00501", "module": "C1", "scenario": "Standard scenario"}, {"value": "0.00315", "module": "C2", "scenario": "Standard scenario"}, {"value": "4.64E-4", "module": "C3", "scenario": "Standard scenario"}, {"value": "5.59E-5", "module": "C4", "scenario": "Standard scenario"}, {"value": "-4.63E-4", "module": "D", "scenario": "Standard scenario"}, {"name": "referenceToUnitGroupDataSet", "value": {"shortDescription": [{"value": "kg"}], "type": "unit group data set", "refObjectId": "ad38d542-3fe9-439d-9b95-2f5f7752acaf", "uri": "../unitgroups/ad38d542-3fe9-439d-9b95-2f5f7752acaf"}}]}, "resolvedFlowVersion": "38.00.000", "flowProperties": [], "typeOfFlow": "Other flow", "classification": {"classHierarchy": "Quantities / Environmental quantities / EPD EN 15804 / LCI indicators", "name": "GaBiCategories"}}, {"dataSetInternalID": 14, "referenceToFlowDataSet": {"shortDescription": [{"value": "Erneuerbare Primärenergie als Energieträger (PERE)", "lang": "de"}, {"value": "Use of renewable primary energy (PERE)", "lang": "en"}, {"value": "Uso de energía primaria renovable excluyendo los recursos de energía primaria renovable utilizada como materia prima (PERE)", "lang": "es"}, {"value": "Förnybar energi - använd som energibärare (PERE)", "lang": "sv"}], "type": "flow data set", "refObjectId": "20f32be5-0398-4288-9b6d-accddd195317", "version": "30.00.001"}, "exchange direction": "INPUT", "meanAmount": 0.0, "other": {"anies": [{"value": "416.0", "module": "A1", "scenario": "Standard scenario"}, {"value": "18.0", "module": "A2", "scenario": "Standard scenario"}, {"value": "113.0", "module": "A3", "scenario": "Standard scenario"}, {"value": "3.9", "module": "C1", "scenario": "Standard scenario"}, {"value": "6.01", "module": "C2", "scenario": "Standard scenario"}, {"value": "5.88", "module": "C3", "scenario": "Standard scenario"}, {"value": "0.0688", "module": "C4", "scenario": "Standard scenario"}, {"value": "1.75", "module": "D", "scenario": "Standard scenario"}, {"name": "referenceToUnitGroupDataSet", "value": {"shortDescription": [{"value": "MJ"}], "type": "unit group data set", "refObjectId": "93a60a57-a3c8-11da-a746-0800200c9a66", "uri": "../unitgroups/93a60a57-a3c8-11da-a746-0800200c9a66"}}]}, "resolvedFlowVersion": "38.00.000", "flowProperties": [], "typeOfFlow": "Other flow", "classification": {"classHierarchy": "Quantities", "name": "GaBiCategories"}}, {"dataSetInternalID": 15, "referenceToFlowDataSet": {"shortDescription": [{"value": "Erneuerbare Primärenergie zur stofflichen Nutzung (PERM)", "lang": "de"}, {"value": "Use of renewable primary energy resources used as raw materials (PERM)", "lang": "en"}, {"value": "Uso de energía primaria renovable utilizada como materia prima (PERM)", "lang": "es"}, {"value": "Förnybar energi - använd som råmaterial (PERM)", "lang": "sv"}], "type": "flow data set", "refObjectId": "fb3ec0de-548d-4508-aea5-00b73bf6f702", "version": "30.00.001"}, "exchange direction": "INPUT", "meanAmount": 0.0, "other": {"anies": [{"value": "0.0", "module": "A1", "scenario": "Standard scenario"}, {"value": "0.0", "module": "A2", "scenario": "Standard scenario"}, {"value": "0.292", "module": "A3", "scenario": "Standard scenario"}, {"value": "0.0", "module": "C1", "scenario": "Standard scenario"}, {"value": "0.0", "module": "C2", "scenario": "Standard scenario"}, {"value": "0.0", "module": "C3", "scenario": "Standard scenario"}, {"value": "0.0", "module": "C4", "scenario": "Standard scenario"}, {"value": "-4.62E-4", "module": "D", "scenario": "Standard scenario"}, {"name": "referenceToUnitGroupDataSet", "value": {"shortDescription": [{"value": "MJ"}], "type": "unit group data set", "refObjectId": "93a60a57-a3c8-11da-a746-0800200c9a66", "uri": "../unitgroups/93a60a57-a3c8-11da-a746-0800200c9a66"}}]}, "resolvedFlowVersion": "38.00.000", "flowProperties": [], "typeOfFlow": "Other flow", "classification": {"classHierarchy": "Quantities", "name": "GaBiCategories"}}, {"dataSetInternalID": 16, "referenceToFlowDataSet": {"shortDescription": [{"value": "Erneuerbare Sekundärbrennstoffe (RSF)", "lang": "de"}, {"value": "Use of renewable secondary fuels (RSF)", "lang": "en"}, {"value": "Uso de combustibles secundarios renovables (RSF)", "lang": "es"}, {"value": "Användning av förnybara sekundära bränslen (RSF)", "lang": "sv"}], "type": "flow data set", "refObjectId": "64333088-a55f-4aa2-9a31-c10b07816787", "version": "30.00.001"}, "exchange direction": "INPUT", "meanAmount": 0.0, "other": {"anies": [{"value": "0.0", "module": "A1", "scenario": "Standard scenario"}, {"value": "0.0", "module": "A2", "scenario": "Standard scenario"}, {"value": "0.0", "module": "A3", "scenario": "Standard scenario"}, {"value": "0.0", "module": "C1", "scenario": "Standard scenario"}, {"value": "0.0", "module": "C2", "scenario": "Standard scenario"}, {"value": "0.0", "module": "C3", "scenario": "Standard scenario"}, {"value": "0.0", "module": "C4", "scenario": "Standard scenario"}, {"value": "0.0", "module": "D", "scenario": "Standard scenario"}, {"name": "referenceToUnitGroupDataSet", "value": {"shortDescription": [{"value": "MJ"}], "type": "unit group data set", "refObjectId": "93a60a57-a3c8-11da-a746-0800200c9a66", "uri": "../unitgroups/93a60a57-a3c8-11da-a746-0800200c9a66"}}]}, "resolvedFlowVersion": "38.00.000", "flowProperties": [], "typeOfFlow": "Other flow", "classification": {"classHierarchy": "Quantities / Environmental quantities / EPD EN 15804 / LCI indicators", "name": "GaBiCategories"}}, {"dataSetInternalID": 17, "referenceToFlowDataSet": {"shortDescription": [{"value": "Einsatz von Sekundärstoffen (SM)", "lang": "de"}, {"value": "Use of secondary material (SM)", "lang": "en"}, {"value": "Uso de materiales secundarios (SM)", "lang": "es"}, {"value": "Användning av sekundära material (SM)", "lang": "sv"}], "type": "flow data set", "refObjectId": "c6a1f35f-2d09-4f54-8dfb-97e502e1ce92", "version": "30.00.001"}, "exchange direction": "INPUT", "meanAmount": 0.0, "other": {"anies": [{"value": "139.0", "module": "A1", "scenario": "Standard scenario"}, {"value": "0.0", "module": "A2", "scenario": "Standard scenario"}, {"value": "0.164", "module": "A3", "scenario": "Standard scenario"}, {"value": "0.0", "module": "C1", "scenario": "Standard scenario"}, {"value": "0.0", "module": "C2", "scenario": "Standard scenario"}, {"value": "0.0", "module": "C3", "scenario": "Standard scenario"}, {"value": "0.0", "module": "C4", "scenario": "Standard scenario"}, {"value": "0.0", "module": "D", "scenario": "Standard scenario"}, {"name": "referenceToUnitGroupDataSet", "value": {"shortDescription": [{"value": "kg"}], "type": "unit group data set", "refObjectId": "ad38d542-3fe9-439d-9b95-2f5f7752acaf", "uri": "../unitgroups/ad38d542-3fe9-439d-9b95-2f5f7752acaf"}}]}, "resolvedFlowVersion": "38.00.000", "flowProperties": [], "typeOfFlow": "Other flow", "classification": {"classHierarchy": "Quantities / Environmental quantities / EPD EN 15804 / LCI indicators", "name": "GaBiCategories"}}, {"dataSetInternalID": 18, "referenceToFlowDataSet": {"shortDescription": [{"value": "Total nicht erneuerbare Primärenergie (PENRT)", "lang": "de"}, {"value": "Total use of non renewable primary energy resource (PENRT)", "lang": "en"}, {"value": "Uso total de la energía primaria no renovable (energía primaria y recursos de energía primaria renovable utilizada como materia prima) (PENRT)", "lang": "es"}, {"value": "Icke förnybar primärenergi – total (PENRT)", "lang": "sv"}], "type": "flow data set", "refObjectId": "06159210-646b-4c8d-8583-da9b3b95a6c1", "version": "30.00.001"}, "exchange direction": "INPUT", "meanAmount": 0.0, "other": {"anies": [{"value": "6330.0", "module": "A1", "scenario": "Standard scenario"}, {"value": "1170.0", "module": "A2", "scenario": "Standard scenario"}, {"value": "1560.0", "module": "A3", "scenario": "Standard scenario"}, {"value": "766.0", "module": "C1", "scenario": "Standard scenario"}, {"value": "510.0", "module": "C2", "scenario": "Standard scenario"}, {"value": "110.0", "module": "C3", "scenario": "Standard scenario"}, {"value": "9.04", "module": "C4", "scenario": "Standard scenario"}, {"value": "-753.0", "module": "D", "scenario": "Standard scenario"}, {"name": "referenceToUnitGroupDataSet", "value": {"shortDescription": [{"value": "MJ"}], "type": "unit group data set", "refObjectId": "93a60a57-a3c8-11da-a746-0800200c9a66", "uri": "../unitgroups/93a60a57-a3c8-11da-a746-0800200c9a66"}}]}, "resolvedFlowVersion": "38.00.000", "flowProperties": [], "typeOfFlow": "Other flow", "classification": {"classHierarchy": "Quantities / Environmental quantities / EPD EN 15804 / LCI indicators", "name": "GaBiCategories"}}, {"dataSetInternalID": 19, "referenceToFlowDataSet": {"shortDescription": [{"value": "Total erneuerbare Primärenergie (PERT)", "lang": "de"}, {"value": "Total use of renewable primary energy resources (PERT)", "lang": "en"}, {"value": "Uso total de la energía primaria renovable (energía primaria y recursos de energía primaria renovable utilizada como materia prima) (PERT)", "lang": "es"}, {"value": "Förnybar energi – total (PERT)", "lang": "sv"}], "type": "flow data set", "refObjectId": "53f97275-fa8a-4cdd-9024-65936002acd0", "version": "30.00.001"}, "exchange direction": "INPUT", "meanAmount": 0.0, "other": {"anies": [{"value": "416.0", "module": "A1", "scenario": "Standard scenario"}, {"value": "18.0", "module": "A2", "scenario": "Standard scenario"}, {"value": "113.0", "module": "A3", "scenario": "Standard scenario"}, {"value": "3.9", "module": "C1", "scenario": "Standard scenario"}, {"value": "6.01", "module": "C2", "scenario": "Standard scenario"}, {"value": "5.88", "module": "C3", "scenario": "Standard scenario"}, {"value": "0.0688", "module": "C4", "scenario": "Standard scenario"}, {"value": "1.75", "module": "D", "scenario": "Standard scenario"}, {"name": "referenceToUnitGroupDataSet", "value": {"shortDescription": [{"value": "MJ"}], "type": "unit group data set", "refObjectId": "93a60a57-a3c8-11da-a746-0800200c9a66", "uri": "../unitgroups/93a60a57-a3c8-11da-a746-0800200c9a66"}}]}, "resolvedFlowVersion": "38.00.000", "flowProperties": [], "typeOfFlow": "Other flow", "classification": {"classHierarchy": "Quantities / Environmental quantities / EPD EN 15804 / LCI indicators", "name": "GaBiCategories"}}]}, "LCIAResults": {"LCIAResult": [{"referenceToLCIAMethodDataSet": {"shortDescription": [{"value": "Potenzial für die Verknappung abiotischer Ressourcen – nicht fossile Ressourcen (ADPE)", "lang": "de"}, {"value": "Abiotic depletion potential - non-fossil resources (ADPE)", "lang": "en"}, {"value": "Abiotisk utarmningspotential icke fossila resurser (ADP-mm)", "lang": "sv"}], "type": "LCIA method data set", "refObjectId": "b2ad6494-c78d-11e6-9d9d-cec0c932ce01", "version": "01.00.012"}, "meanAmount": 0.0, "other": {"anies": [{"value": "0.00444", "module": "A1", "scenario": "Standard scenario"}, {"value": "0.00144", "module": "A2", "scenario": "Standard scenario"}, {"value": "3.03E-4", "module": "A3", "scenario": "Standard scenario"}, {"value": "8.03E-5", "module": "C1", "scenario": "Standard scenario"}, {"value": "8.06E-4", "module": "C2", "scenario": "Standard scenario"}, {"value": "2.17E-5", "module": "C3", "scenario": "Standard scenario"}, {"value": "2.79E-6", "module": "C4", "scenario": "Standard scenario"}, {"value": "-0.00107", "module": "D", "scenario": "Standard scenario"}, {"name": "referenceToUnitGroupDataSet", "value": {"shortDescription": [{"value": "kg Sb-Äqv."}], "type": "unit group data set", "refObjectId": "54ccd2d9-a32a-4fc2-923d-f2c8c93e89d4", "uri": "../unitgroups/54ccd2d9-a32a-4fc2-923d-f2c8c93e89d4"}}]}}, {"referenceToLCIAMethodDataSet": {"shortDescription": [{"value": "Potenzial für die Verknappung abiotischer Ressourcen – fossile Brennstoffe (ADPF)", "lang": "de"}, {"value": "Abiotic depletion potential - fossil resources (ADPF)", "lang": "en"}, {"value": "Abiotisk utarmningspotential av fossila resurser (ADP-F)", "lang": "sv"}], "type": "LCIA method data set", "refObjectId": "b2ad6110-c78d-11e6-9d9d-cec0c932ce01", "version": "01.00.012"}, "meanAmount": 0.0, "other": {"anies": [{"value": "5980.0", "module": "A1", "scenario": "Standard scenario"}, {"value": "1100.0", "module": "A2", "scenario": "Standard scenario"}, {"value": "1440.0", "module": "A3", "scenario": "Standard scenario"}, {"value": "721.0", "module": "C1", "scenario": "Standard scenario"}, {"value": "480.0", "module": "C2", "scenario": "Standard scenario"}, {"value": "103.0", "module": "C3", "scenario": "Standard scenario"}, {"value": "8.51", "module": "C4", "scenario": "Standard scenario"}, {"value": "-722.0", "module": "D", "scenario": "Standard scenario"}, {"name": "referenceToUnitGroupDataSet", "value": {"shortDescription": [{"value": "MJ"}], "type": "unit group data set", "refObjectId": "93a60a57-a3c8-11da-a746-0800200c9a66", "uri": "../unitgroups/93a60a57-a3c8-11da-a746-0800200c9a66"}}]}}, {"referenceToLCIAMethodDataSet": {"shortDescription": [{"value": "Versauerungspotenzial, kumulierte Überschreitung (AP)", "lang": "de"}, {"value": "Acidification potential, Accumulated Exceedance (AP)", "lang": "en"}, {"value": "Försurningspotential på land och vatten (AP)", "lang": "sv"}], "type": "LCIA method data set", "refObjectId": "b5c611c6-def3-11e6-bf01-fe55135034f3", "version": "01.03.011", "uri": "http://lca.jrc.ec.europa.eu/lcainfohub/datasets/elcd/lciamethods/f6cbd466-253f-4145-a4bb-8dae7d266e89.xml"}, "meanAmount": 0.0, "other": {"anies": [{"value": "2.85", "module": "A1", "scenario": "Standard scenario"}, {"value": "0.577", "module": "A2", "scenario": "Standard scenario"}, {"value": "0.258", "module": "A3", "scenario": "Standard scenario"}, {"value": "0.548", "module": "C1", "scenario": "Standard scenario"}, {"value": "0.185", "module": "C2", "scenario": "Standard scenario"}, {"value": "0.0483", "module": "C3", "scenario": "Standard scenario"}, {"value": "0.00289", "module": "C4", "scenario": "Standard scenario"}, {"value": "-0.415", "module": "D", "scenario": "Standard scenario"}, {"name": "referenceToUnitGroupDataSet", "value": {"shortDescription": [{"value": "mol H+ eqv."}], "type": "unit group data set", "refObjectId": "42e089ac-92bf-4bf2-8ca1-5fc40d18f2ed", "uri": "../unitgroups/42e089ac-92bf-4bf2-8ca1-5fc40d18f2ed"}}]}}, {"referenceToLCIAMethodDataSet": {"shortDescription": [{"value": "Eutrophierungspotenzial - Süßwasser (EP-freshwater)", "lang": "de"}, {"value": "Eutrophication potential - freshwater (EP-freshwater)", "lang": "en"}, {"value": "Övergödningspotential sötvatten (EP-fw)", "lang": "sv"}], "type": "LCIA method data set", "refObjectId": "b53ec18f-7377-4ad3-86eb-cc3f4f276b2b", "version": "01.00.012", "uri": "http://lca.jrc.ec.europa.eu/lcainfohub/datasets/elcd/lciamethods/a4630d5b-df2f-48ae-b3f2-5e5257606d68.xml"}, "meanAmount": 0.0, "other": {"anies": [{"value": "0.0212", "module": "A1", "scenario": "Standard scenario"}, {"value": "8.45E-4", "module": "A2", "scenario": "Standard scenario"}, {"value": "0.0103", "module": "A3", "scenario": "Standard scenario"}, {"value": "1.91E-4", "module": "C1", "scenario": "Standard scenario"}, {"value": "3.21E-4", "module": "C2", "scenario": "Standard scenario"}, {"value": "2.4E-4", "module": "C3", "scenario": "Standard scenario"}, {"value": "3.41E-6", "module": "C4", "scenario": "Standard scenario"}, {"value": "-0.00317", "module": "D", "scenario": "Standard scenario"}, {"name": "referenceToUnitGroupDataSet", "value": {"shortDescription": [{"value": "kg P eqv."}], "type": "unit group data set", "refObjectId": "0429039d-a61d-4590-ba67-aa4a20a810a1", "uri": "../unitgroups/0429039d-a61d-4590-ba67-aa4a20a810a1"}}]}}, {"referenceToLCIAMethodDataSet": {"shortDescription": [{"value": "Eutrophierungspotenzial - Salzwasser (EP-marine)", "lang": "de"}, {"value": "Eutrophication potential - marine (EP-marine)", "lang": "en"}, {"value": "Övergödningspotential marin (EP-m)", "lang": "sv"}], "type": "LCIA method data set", "refObjectId": "b5c619fa-def3-11e6-bf01-fe55135034f3", "version": "02.00.012", "uri": "http://lca.jrc.ec.europa.eu/lcainfohub/datasets/elcd/lciamethods/5296e2be-060b-4e50-b033-d45f85f6ac92.xml"}, "meanAmount": 0.0, "other": {"anies": [{"value": "0.681", "module": "A1", "scenario": "Standard scenario"}, {"value": "0.226", "module": "A2", "scenario": "Standard scenario"}, {"value": "0.0658", "module": "A3", "scenario": "Standard scenario"}, {"value": "0.242", "module": "C1", "scenario": "Standard scenario"}, {"value": "0.065", "module": "C2", "scenario": "Standard scenario"}, {"value": "0.0192", "module": "C3", "scenario": "Standard scenario"}, {"value": "9.94E-4", "module": "C4", "scenario": "Standard scenario"}, {"value": "-0.0925", "module": "D", "scenario": "Standard scenario"}, {"name": "referenceToUnitGroupDataSet", "value": {"shortDescription": [{"value": "kg N eqv."}], "type": "unit group data set", "refObjectId": "d05bb823-ecdf-4686-8c40-bf1d9257859f", "uri": "../unitgroups/d05bb823-ecdf-4686-8c40-bf1d9257859f"}}]}}, {"referenceToLCIAMethodDataSet": {"shortDescription": [{"value": "Eutrophierungspotenzial - Land (EP-terrestrial)", "lang": "de"}, {"value": "Eutrophication potential - terrestrial (EP-terrestrial)", "lang": "en"}, {"value": "Övergödningspotential total (EP-T)", "lang": "sv"}], "type": "LCIA method data set", "refObjectId": "b5c614d2-def3-11e6-bf01-fe55135034f3", "version": "01.02.011", "uri": "http://lca.jrc.ec.europa.eu/lcainfohub/datasets/elcd/lciamethods/40054970-5936-477c-9bec-29fa23b1cb77.xml"}, "meanAmount": 0.0, "other": {"anies": [{"value": "7.87", "module": "A1", "scenario": "Standard scenario"}, {"value": "2.49", "module": "A2", "scenario": "Standard scenario"}, {"value": "0.778", "module": "A3", "scenario": "Standard scenario"}, {"value": "2.65", "module": "C1", "scenario": "Standard scenario"}, {"value": "0.717", "module": "C2", "scenario": "Standard scenario"}, {"value": "0.213", "module": "C3", "scenario": "Standard scenario"}, {"value": "0.011", "module": "C4", "scenario": "Standard scenario"}, {"value": "-1.08", "module": "D", "scenario": "Standard scenario"}, {"name": "referenceToUnitGroupDataSet", "value": {"shortDescription": [{"value": "mol N eqv."}], "type": "unit group data set", "refObjectId": "71b4d617-0ec9-4d3f-b65e-e438940c2401", "uri": "../unitgroups/71b4d617-0ec9-4d3f-b65e-e438940c2401"}}]}}, {"referenceToLCIAMethodDataSet": {"shortDescription": [{"value": "Globales Erwärmungspotenzial - total (GWP-total)", "lang": "de"}, {"value": "Global Warming Potential - total (GWP-total)", "lang": "en"}, {"value": "Global uppvärmningspotential – Totalt (GWP-T)", "lang": "sv"}], "type": "LCIA method data set", "refObjectId": "6a37f984-a4b3-458a-a20a-64418c145fa2", "version": "04.00.018"}, "meanAmount": 0.0, "other": {"anies": [{"value": "935.0", "module": "A1", "scenario": "Standard scenario"}, {"value": "78.0", "module": "A2", "scenario": "Standard scenario"}, {"value": "110.0", "module": "A3", "scenario": "Standard scenario"}, {"value": "52.4", "module": "C1", "scenario": "Standard scenario"}, {"value": "31.8", "module": "C2", "scenario": "Standard scenario"}, {"value": "7.74", "module": "C3", "scenario": "Standard scenario"}, {"value": "0.305", "module": "C4", "scenario": "Standard scenario"}, {"value": "-91.9", "module": "D", "scenario": "Standard scenario"}, {"name": "referenceToUnitGroupDataSet", "value": {"shortDescription": [{"value": "kg CO2-Äqv."}], "type": "unit group data set", "refObjectId": "1ebf3012-d0db-4de2-aefd-ef30cedb0be1", "uri": "../unitgroups/1ebf3012-d0db-4de2-aefd-ef30cedb0be1"}}]}}, {"referenceToLCIAMethodDataSet": {"shortDescription": [{"value": "Globales Erwärmungspotenzial - fossil (GWP-fossil)", "lang": "de"}, {"value": "Global Warming Potential - fossil fuels (GWP-fossil)", "lang": "en"}, {"value": "Global uppvärmningspotential– fossil (GWP-f)", "lang": "sv"}], "type": "LCIA method data set", "refObjectId": "5f635281-343e-44fb-83df-1971b155e6b6", "version": "01.00.011"}, "meanAmount": 0.0, "other": {"anies": [{"value": "923.0", "module": "A1", "scenario": "Standard scenario"}, {"value": "77.9", "module": "A2", "scenario": "Standard scenario"}, {"value": "105.0", "module": "A3", "scenario": "Standard scenario"}, {"value": "52.4", "module": "C1", "scenario": "Standard scenario"}, {"value": "31.8", "module": "C2", "scenario": "Standard scenario"}, {"value": "7.7", "module": "C3", "scenario": "Standard scenario"}, {"value": "0.304", "module": "C4", "scenario": "Standard scenario"}, {"value": "-92.7", "module": "D", "scenario": "Standard scenario"}, {"name": "referenceToUnitGroupDataSet", "value": {"shortDescription": [{"value": "kg CO2-Äqv."}], "type": "unit group data set", "refObjectId": "1ebf3012-d0db-4de2-aefd-ef30cedb0be1", "uri": "../unitgroups/1ebf3012-d0db-4de2-aefd-ef30cedb0be1"}}]}}, {"referenceToLCIAMethodDataSet": {"shortDescription": [{"value": "Globales Erwärmungspotenzial - biogen (GWP-biogenic)", "lang": "de"}, {"value": "Global Warming Potential - biogenic (GWP-biogenic)", "lang": "en"}, {"value": "Global uppvärmningspotential – biogen (GWP-b)", "lang": "sv"}], "type": "LCIA method data set", "refObjectId": "2356e1ab-0185-4db5-86e5-16de51c7485c", "version": "01.00.007"}, "meanAmount": 0.0, "other": {"anies": [{"value": "11.3", "module": "A1", "scenario": "Standard scenario"}, {"value": "0.0712", "module": "A2", "scenario": "Standard scenario"}, {"value": "5.42", "module": "A3", "scenario": "Standard scenario"}, {"value": "0.0146", "module": "C1", "scenario": "Standard scenario"}, {"value": "0.0147", "module": "C2", "scenario": "Standard scenario"}, {"value": "0.0445", "module": "C3", "scenario": "Standard scenario"}, {"value": "6.04E-4", "module": "C4", "scenario": "Standard scenario"}, {"value": "0.708", "module": "D", "scenario": "Standard scenario"}, {"name": "referenceToUnitGroupDataSet", "value": {"shortDescription": [{"value": "kg CO2-Äqv."}], "type": "unit group data set", "refObjectId": "1ebf3012-d0db-4de2-aefd-ef30cedb0be1", "uri": "../unitgroups/1ebf3012-d0db-4de2-aefd-ef30cedb0be1"}}]}}, {"referenceToLCIAMethodDataSet": {"shortDescription": [{"value": "Globales Erwärmungspotenzial - luluc (GWP-luluc)", "lang": "de"}, {"value": "Global Warming Potential - land use and land use change (GWP-luluc)", "lang": "en"}, {"value": "Global uppvärmningspotential - markanvändning och förändringar i markanvändning (GWP-luluc)", "lang": "sv"}], "type": "LCIA method data set", "refObjectId": "4331bbdb-978a-490d-8707-eeb047f01a55", "version": "01.00.007"}, "meanAmount": 0.0, "other": {"anies": [{"value": "0.302", "module": "A1", "scenario": "Standard scenario"}, {"value": "0.074", "module": "A2", "scenario": "Standard scenario"}, {"value": "0.081", "module": "A3", "scenario": "Standard scenario"}, {"value": "0.00413", "module": "C1", "scenario": "Standard scenario"}, {"value": "0.0117", "module": "C2", "scenario": "Standard scenario"}, {"value": "0.00146", "module": "C3", "scenario": "Standard scenario"}, {"value": "8.49E-5", "module": "C4", "scenario": "Standard scenario"}, {"value": "0.0425", "module": "D", "scenario": "Standard scenario"}, {"name": "referenceToUnitGroupDataSet", "value": {"shortDescription": [{"value": "kg CO2-Äqv."}], "type": "unit group data set", "refObjectId": "1ebf3012-d0db-4de2-aefd-ef30cedb0be1", "uri": "../unitgroups/1ebf3012-d0db-4de2-aefd-ef30cedb0be1"}}]}}, {"referenceToLCIAMethodDataSet": {"shortDescription": [{"value": "Abbaupotenzial der stratosphärischen Ozonschicht (ODP)", "lang": "de"}, {"value": "Depletion potential of the stratospheric ozone layer (ODP)", "lang": "en"}, {"value": "Utarmningspotential för stratosfäriska ozonskiktet - ozonnedbrytning (ODP)", "lang": "sv"}], "type": "LCIA method data set", "refObjectId": "b5c629d6-def3-11e6-bf01-fe55135034f3", "version": "02.00.014", "uri": "http://lca.jrc.ec.europa.eu/lcainfohub/datasets/elcd/lciamethods/8b723200-3d8f-4eec-9e10-444edb029476.xml"}, "meanAmount": 0.0, "other": {"anies": [{"value": "4.25E-5", "module": "A1", "scenario": "Standard scenario"}, {"value": "1.58E-5", "module": "A2", "scenario": "Standard scenario"}, {"value": "7.9E-6", "module": "A3", "scenario": "Standard scenario"}, {"value": "1.13E-5", "module": "C1", "scenario": "Standard scenario"}, {"value": "7.02E-6", "module": "C2", "scenario": "Standard scenario"}, {"value": "9.98E-7", "module": "C3", "scenario": "Standard scenario"}, {"value": "1.25E-7", "module": "C4", "scenario": "Standard scenario"}, {"value": "-3.54E-6", "module": "D", "scenario": "Standard scenario"}, {"name": "referenceToUnitGroupDataSet", "value": {"shortDescription": [{"value": "kg CFC 11-Äquiv."}], "type": "unit group data set", "refObjectId": "d9e957c9-7309-4474-bf3a-7777df6c4e5b", "uri": "../unitgroups/d9e957c9-7309-4474-bf3a-7777df6c4e5b"}}]}}, {"referenceToLCIAMethodDataSet": {"shortDescription": [{"value": "Bildungspotenzial für troposphärisches Ozon (POCP)", "lang": "de"}, {"value": "Photochemical Ozone Creation Potential (POCP)", "lang": "en"}, {"value": "Potential till fotokemisk oxidantbildning – marknära ozon (POCP)", "lang": "sv"}], "type": "LCIA method data set", "refObjectId": "b5c610fe-def3-11e6-bf01-fe55135034f3", "version": "02.00.017", "uri": "http://lca.jrc.ec.europa.eu/lcainfohub/datasets/elcd/lciamethods/ec7836be-83eb-41da-bcda-1a6a3fe2d149.xml"}, "meanAmount": 0.0, "other": {"anies": [{"value": "2.48", "module": "A1", "scenario": "Standard scenario"}, {"value": "0.672", "module": "A2", "scenario": "Standard scenario"}, {"value": "0.178", "module": "A3", "scenario": "Standard scenario"}, {"value": "0.73", "module": "C1", "scenario": "Standard scenario"}, {"value": "0.205", "module": "C2", "scenario": "Standard scenario"}, {"value": "0.058", "module": "C3", "scenario": "Standard scenario"}, {"value": "0.00318", "module": "C4", "scenario": "Standard scenario"}, {"value": "-0.55", "module": "D", "scenario": "Standard scenario"}, {"name": "referenceToUnitGroupDataSet", "value": {"shortDescription": [{"value": "kg NMVOC eqv."}], "type": "unit group data set", "refObjectId": "d27c25f8-fbc1-44c6-b47b-4adbae4199c6", "uri": "../unitgroups/d27c25f8-fbc1-44c6-b47b-4adbae4199c6"}}]}}, {"referenceToLCIAMethodDataSet": {"shortDescription": [{"value": "Wasser-Entzugspotenzial (Benutzer) (WDP)", "lang": "de"}, {"value": "Water (user) deprivation potential (WDP)", "lang": "en"}, {"value": "Vattenfotavtryck (WDP)", "lang": "sv"}], "type": "LCIA method data set", "refObjectId": "b2ad66ce-c78d-11e6-9d9d-cec0c932ce01", "version": "03.00.016"}, "meanAmount": 0.0, "other": {"anies": [{"value": "296.0", "module": "A1", "scenario": "Standard scenario"}, {"value": "4.38", "module": "A2", "scenario": "Standard scenario"}, {"value": "3.73", "module": "A3", "scenario": "Standard scenario"}, {"value": "0.966", "module": "C1", "scenario": "Standard scenario"}, {"value": "1.72", "module": "C2", "scenario": "Standard scenario"}, {"value": "0.469", "module": "C3", "scenario": "Standard scenario"}, {"value": "0.381", "module": "C4", "scenario": "Standard scenario"}, {"value": "-309.0", "module": "D", "scenario": "Standard scenario"}, {"name": "referenceToUnitGroupDataSet", "value": {"shortDescription": [{"value": "m3 world eqv."}], "type": "unit group data set", "refObjectId": "6ae2df01-888e-46c8-b17d-49fa3869b476", "uri": "../unitgroups/6ae2df01-888e-46c8-b17d-49fa3869b476"}}]}}, {"referenceToLCIAMethodDataSet": {"shortDescription": [{"value": "Potenzielles Auftreten von Krankheiten aufgrund von Feinstaubemissionen (PM)", "lang": "de"}, {"value": "Potential incidence of disease due to PM emissions (PM)", "lang": "en"}, {"value": "Potential till utsläpp av partiklar (PM)", "lang": "sv"}], "type": "LCIA method data set", "refObjectId": "b5c602c6-def3-11e6-bf01-fe55135034f3", "version": "02.00.013", "uri": "http://lca.jrc.ec.europa.eu/lcainfohub/datasets/elcd/lciamethods/72ce3013-f678-4c6a-935b-f4752ff8901b.xml"}, "meanAmount": 0.0, "other": {"anies": [{"value": "3.22E-5", "module": "A1", "scenario": "Standard scenario"}, {"value": "4.97E-6", "module": "A2", "scenario": "Standard scenario"}, {"value": "1.87E-6", "module": "A3", "scenario": "Standard scenario"}, {"value": "1.45E-5", "module": "C1", "scenario": "Standard scenario"}, {"value": "2.86E-6", "module": "C2", "scenario": "Standard scenario"}, {"value": "1.07E-6", "module": "C3", "scenario": "Standard scenario"}, {"value": "5.62E-8", "module": "C4", "scenario": "Standard scenario"}, {"value": "-6.39E-6", "module": "D", "scenario": "Standard scenario"}, {"name": "referenceToUnitGroupDataSet", "value": {"shortDescription": [{"value": "disease incidence"}], "type": "unit group data set", "refObjectId": "3883559b-648f-4afc-8ba2-0bd24f3affa3", "uri": "../unitgroups/3883559b-648f-4afc-8ba2-0bd24f3affa3"}}]}}, {"referenceToLCIAMethodDataSet": {"shortDescription": [{"value": "Potenzielle Wirkung durch Exposition des Menschen mit U235 (IRP)", "lang": "de"}, {"value": "Potential Human exposure efficiency relative to U235 (IRP)", "lang": "en"}, {"value": "Exponeringseffektivitet relaterad till U235 (IR)", "lang": "sv"}], "type": "LCIA method data set", "refObjectId": "b5c632be-def3-11e6-bf01-fe55135034f3", "version": "01.00.013", "uri": "http://lca.jrc.ec.europa.eu/lcainfohub/datasets/elcd/lciamethods/a6f4cbc8-5388-44d6-9a67-53d05684f93e.xml"}, "meanAmount": 0.0, "other": {"anies": [{"value": "23.6", "module": "A1", "scenario": "Standard scenario"}, {"value": "4.67", "module": "A2", "scenario": "Standard scenario"}, {"value": "3.42", "module": "A3", "scenario": "Standard scenario"}, {"value": "3.09", "module": "C1", "scenario": "Standard scenario"}, {"value": "2.01", "module": "C2", "scenario": "Standard scenario"}, {"value": "0.328", "module": "C3", "scenario": "Standard scenario"}, {"value": "0.0349", "module": "C4", "scenario": "Standard scenario"}, {"value": "0.535", "module": "D", "scenario": "Standard scenario"}, {"name": "referenceToUnitGroupDataSet", "value": {"shortDescription": [{"value": "kBq U235 eqv."}], "type": "unit group data set", "refObjectId": "456b05bf-1415-44a9-9993-02452f554c09", "uri": "../unitgroups/456b05bf-1415-44a9-9993-02452f554c09"}}]}}, {"referenceToLCIAMethodDataSet": {"shortDescription": [{"value": "Potenzielle Toxizitätsvergleichseinheit für Ökosysteme (ETP-fw)", "lang": "de"}, {"value": "Potential Comparative Toxic Unit for ecosystems (ETP-fw)", "lang": "en"}, {"value": "Ecotoxicitet (ETP-fw) ", "lang": "sv"}], "type": "LCIA method data set", "refObjectId": "ee1082d1-b0f7-43ca-a1f0-21e2a4a74511", "version": "01.00.004", "uri": "http://lca.jrc.ec.europa.eu/lcainfohub/datasets/elcd/lciamethods/ee1082d1-b0f7-43ca-a1f0-21e2a4a74511.xml"}, "meanAmount": 0.0, "other": {"anies": [{"value": "11900.0", "module": "A1", "scenario": "Standard scenario"}, {"value": "979.0", "module": "A2", "scenario": "Standard scenario"}, {"value": "884.0", "module": "A3", "scenario": "Standard scenario"}, {"value": "435.0", "module": "C1", "scenario": "Standard scenario"}, {"value": "428.0", "module": "C2", "scenario": "Standard scenario"}, {"value": "83.8", "module": "C3", "scenario": "Standard scenario"}, {"value": "5.52", "module": "C4", "scenario": "Standard scenario"}, {"value": "-2860.0", "module": "D", "scenario": "Standard scenario"}, {"name": "referenceToUnitGroupDataSet", "value": {"shortDescription": [{"value": "CTUe"}], "type": "unit group data set", "refObjectId": "aa959ded-f1eb-4efb-9c5c-2d60be36b3e6", "uri": "../unitgroups/aa959ded-f1eb-4efb-9c5c-2d60be36b3e6"}}]}}, {"referenceToLCIAMethodDataSet": {"shortDescription": [{"value": "Potenzielle Toxizitätsvergleichseinheit für den Menschen - kanzerogene Wirkung (HTP-c)", "lang": "de"}, {"value": "Potential Comparative Toxic Unit for humans - cancer effects (HTP-c)", "lang": "en"}, {"value": "Humantoxicitet – cancer (HTP-c)", "lang": "sv"}], "type": "LCIA method data set", "refObjectId": "2299222a-bbd8-474f-9d4f-4dd1f18aea7c", "version": "01.00.005", "uri": "http://lca.jrc.ec.europa.eu/lcainfohub/datasets/elcd/lciamethods/2299222a-bbd8-474f-9d4f-4dd1f18aea7c.xml"}, "meanAmount": 0.0, "other": {"anies": [{"value": "2.24E-6", "module": "A1", "scenario": "Standard scenario"}, {"value": "3.51E-8", "module": "A2", "scenario": "Standard scenario"}, {"value": "2.44E-8", "module": "A3", "scenario": "Standard scenario"}, {"value": "1.52E-8", "module": "C1", "scenario": "Standard scenario"}, {"value": "1.39E-8", "module": "C2", "scenario": "Standard scenario"}, {"value": "1.99E-9", "module": "C3", "scenario": "Standard scenario"}, {"value": "1.28E-10", "module": "C4", "scenario": "Standard scenario"}, {"value": "3.96E-8", "module": "D", "scenario": "Standard scenario"}, {"name": "referenceToUnitGroupDataSet", "value": {"shortDescription": [{"value": "CTUh"}], "type": "unit group data set", "refObjectId": "d4c9523e-2d7e-49fd-8469-998f547d3a70", "uri": "../unitgroups/d4c9523e-2d7e-49fd-8469-998f547d3a70"}}]}}, {"referenceToLCIAMethodDataSet": {"shortDescription": [{"value": "Potenzielle Toxizitätsvergleichseinheit für den Menschen - nicht kanzerogene Wirkung (HTP-nc)", "lang": "de"}, {"value": "Potential Comparative Toxic Unit for humans - non-cancer effects (HTP-nc)", "lang": "en"}, {"value": "Humantoxicitet – icke cancer (HTP-nc)", "lang": "sv"}], "type": "LCIA method data set", "refObjectId": "3af763a5-b7a1-48c9-9cee-1f223481fcef", "version": "01.00.004", "uri": "http://lca.jrc.ec.europa.eu/lcainfohub/datasets/elcd/lciamethods/3af763a5-b7a1-48c9-9cee-1f223481fcef.xml"}, "meanAmount": 0.0, "other": {"anies": [{"value": "5.01E-5", "module": "A1", "scenario": "Standard scenario"}, {"value": "9.32E-7", "module": "A2", "scenario": "Standard scenario"}, {"value": "8.03E-7", "module": "A3", "scenario": "Standard scenario"}, {"value": "3.73E-7", "module": "C1", "scenario": "Standard scenario"}, {"value": "4.68E-7", "module": "C2", "scenario": "Standard scenario"}, {"value": "5.62E-8", "module": "C3", "scenario": "Standard scenario"}, {"value": "3.92E-9", "module": "C4", "scenario": "Standard scenario"}, {"value": "1.64E-5", "module": "D", "scenario": "Standard scenario"}, {"name": "referenceToUnitGroupDataSet", "value": {"shortDescription": [{"value": "CTUh"}], "type": "unit group data set", "refObjectId": "d4c9523e-2d7e-49fd-8469-998f547d3a70", "uri": "../unitgroups/d4c9523e-2d7e-49fd-8469-998f547d3a70"}}]}}, {"referenceToLCIAMethodDataSet": {"shortDescription": [{"value": "Potenzieller Bodenqualitätsindex (SQP)", "lang": "de"}, {"value": "Potential Soil quality index (SQP)", "lang": "en"}, {"value": "Potentiell jordkvalitet index (SQP)", "lang": "sv"}], "type": "LCIA method data set", "refObjectId": "b2ad6890-c78d-11e6-9d9d-cec0c932ce01", "version": "01.00.014"}, "meanAmount": 0.0, "other": {"anies": [{"value": "1880.0", "module": "A1", "scenario": "Standard scenario"}, {"value": "916.0", "module": "A2", "scenario": "Standard scenario"}, {"value": "199.0", "module": "A3", "scenario": "Standard scenario"}, {"value": "92.0", "module": "C1", "scenario": "Standard scenario"}, {"value": "416.0", "module": "C2", "scenario": "Standard scenario"}, {"value": "17.3", "module": "C3", "scenario": "Standard scenario"}, {"value": "17.8", "module": "C4", "scenario": "Standard scenario"}, {"value": "-434.0", "module": "D", "scenario": "Standard scenario"}, {"name": "referenceToUnitGroupDataSet", "value": {"shortDescription": [{"value": "dimensionless"}], "type": "unit group data set", "refObjectId": "f130951c-e67f-4f7f-8dd4-665de3974e18", "uri": "../unitgroups/f130951c-e67f-4f7f-8dd4-665de3974e18"}}]}}]}, "otherAttributes": {"{http://www.okworx.com/ILCD/Extensions/2018/Profile}profile": "EN_15804_A2", "{http://www.indata.network/EPD/2019}epd-version": "1.2"}, "version": "1.1"}