{"processInformation": {"dataSetInformation": {"UUID": "c2c26b16-ac23-4cc8-a8d1-709fbe2f7cc2", "name": {"baseName": [{"value": "Schiedel SIH Parat (Chimney System)", "lang": "en"}, {"value": "Schiedel SIH Parat (Schornsteinsystem)", "lang": "de"}]}, "classificationInformation": {"classification": [{"class": [{"value": "Komponenten von Fenstern und Vorhangfassaden", "level": 0, "classId": "7"}, {"value": "Tageslichtsysteme und Rauch- / Wärmeabzugsanlagen ", "level": 1, "classId": "7.10"}, {"value": "Rauch-/Wärmeabzugsanlagen", "level": 2, "classId": "7.10.02"}], "name": "OEKOBAU.DAT"}]}, "generalComment": [{"value": "Schiedel SIH Parat is a product of the SIH chimney product series. The producer and distributor is Schiedel GmbH & Co. KG, based in Munich (Germany). The EPD refers to the specific product SIH Parat single duct without ventilation/installation. EPD type: Cradle to gate with modules C1-C4 and module D. Kiwa-Ecobility Experts shall not be liable with respect to manufacturer information, life cycle assessment data and evidence.", "lang": "en"}], "other": {"anies": [{"scenario": [{"description": [{"value": "The most datasets chosen for the LCA refer to Germany as the geographic reference. If this was not available, datasets from EU or Switzerland were chosen. Transport distances for all raw materials used could be recorded. A payload factor of 50 percent was used for all truck transports (suppliers, disposal transports and internal transports), which corresponds to a full delivery and empty return trip. A data set for a non-specific truck was used. Electricity mix was modeled according to the information provided by the company. For some raw materials, no specific datasets were available the EcoInvent database, and alternatives were chosen. For demolition (module C1) a general dataset on machine operation was chosen, which according to EcoInvent represents an average for different construction site machines and/or processes such as cranes, rammers or crushing. It has been assumed that for the demolition of a chimney of a standard length one hour is needed. For the end-of-life it has been assumed that the product is 100% landfilled. Note: The transport distances of the waste are based on the standard waste scenarios of the NMD Determination Method (NMD 2019): incineration 150 km/ recycling 50 km / landfill 100 km; vehicle: truck, unspecific. For all transports, the environmental profile of a non-specific truck transport was used (conservative assumption): The vehicle operates with diesel, and it provides a fleet average that includes different lorry classes as well as EURO classes. This environmental profile contains data for transport, which is calculated for an average load factor, including empty return trips (EcoInvent 3.6)."}], "name": "Standard scenario", "default": true}]}, "<ns11:modules xmlns:ns11=\"http://openlca.org/epd_ilcd\" xmlns=\"http://lca.jrc.it/ILCD/Process\" xmlns:c=\"http://lca.jrc.it/ILCD/Contact\" xmlns:common=\"http://lca.jrc.it/ILCD/Common\" xmlns:epd=\"http://www.iai.kit.edu/EPD/2013\" xmlns:epd2=\"http://www.indata.network/EPD/2019\" xmlns:f=\"http://lca.jrc.it/ILCD/Flow\" xmlns:fp=\"http://lca.jrc.it/ILCD/FlowProperty\" xmlns:m=\"http://lca.jrc.it/ILCD/LCIAMethod\" xmlns:ns9=\"http://www.okworx.com/ILCD/Extensions/2018/Profile\" xmlns:s=\"http://lca.jrc.it/ILCD/Source\" xmlns:u=\"http://lca.jrc.it/ILCD/UnitGroup\" name=\"A1\" scenario=\"Standard scenario\"/>", "<ns11:modules xmlns:ns11=\"http://openlca.org/epd_ilcd\" xmlns=\"http://lca.jrc.it/ILCD/Process\" xmlns:c=\"http://lca.jrc.it/ILCD/Contact\" xmlns:common=\"http://lca.jrc.it/ILCD/Common\" xmlns:epd=\"http://www.iai.kit.edu/EPD/2013\" xmlns:epd2=\"http://www.indata.network/EPD/2019\" xmlns:f=\"http://lca.jrc.it/ILCD/Flow\" xmlns:fp=\"http://lca.jrc.it/ILCD/FlowProperty\" xmlns:m=\"http://lca.jrc.it/ILCD/LCIAMethod\" xmlns:ns9=\"http://www.okworx.com/ILCD/Extensions/2018/Profile\" xmlns:s=\"http://lca.jrc.it/ILCD/Source\" xmlns:u=\"http://lca.jrc.it/ILCD/UnitGroup\" name=\"A2\" scenario=\"Standard scenario\"/>", "<ns11:modules xmlns:ns11=\"http://openlca.org/epd_ilcd\" xmlns=\"http://lca.jrc.it/ILCD/Process\" xmlns:c=\"http://lca.jrc.it/ILCD/Contact\" xmlns:common=\"http://lca.jrc.it/ILCD/Common\" xmlns:epd=\"http://www.iai.kit.edu/EPD/2013\" xmlns:epd2=\"http://www.indata.network/EPD/2019\" xmlns:f=\"http://lca.jrc.it/ILCD/Flow\" xmlns:fp=\"http://lca.jrc.it/ILCD/FlowProperty\" xmlns:m=\"http://lca.jrc.it/ILCD/LCIAMethod\" xmlns:ns9=\"http://www.okworx.com/ILCD/Extensions/2018/Profile\" xmlns:s=\"http://lca.jrc.it/ILCD/Source\" xmlns:u=\"http://lca.jrc.it/ILCD/UnitGroup\" name=\"A3\" scenario=\"Standard scenario\"/>", "<ns11:modules xmlns:ns11=\"http://openlca.org/epd_ilcd\" xmlns=\"http://lca.jrc.it/ILCD/Process\" xmlns:c=\"http://lca.jrc.it/ILCD/Contact\" xmlns:common=\"http://lca.jrc.it/ILCD/Common\" xmlns:epd=\"http://www.iai.kit.edu/EPD/2013\" xmlns:epd2=\"http://www.indata.network/EPD/2019\" xmlns:f=\"http://lca.jrc.it/ILCD/Flow\" xmlns:fp=\"http://lca.jrc.it/ILCD/FlowProperty\" xmlns:m=\"http://lca.jrc.it/ILCD/LCIAMethod\" xmlns:ns9=\"http://www.okworx.com/ILCD/Extensions/2018/Profile\" xmlns:s=\"http://lca.jrc.it/ILCD/Source\" xmlns:u=\"http://lca.jrc.it/ILCD/UnitGroup\" name=\"C1\" scenario=\"Standard scenario\"/>", "<ns11:modules xmlns:ns11=\"http://openlca.org/epd_ilcd\" xmlns=\"http://lca.jrc.it/ILCD/Process\" xmlns:c=\"http://lca.jrc.it/ILCD/Contact\" xmlns:common=\"http://lca.jrc.it/ILCD/Common\" xmlns:epd=\"http://www.iai.kit.edu/EPD/2013\" xmlns:epd2=\"http://www.indata.network/EPD/2019\" xmlns:f=\"http://lca.jrc.it/ILCD/Flow\" xmlns:fp=\"http://lca.jrc.it/ILCD/FlowProperty\" xmlns:m=\"http://lca.jrc.it/ILCD/LCIAMethod\" xmlns:ns9=\"http://www.okworx.com/ILCD/Extensions/2018/Profile\" xmlns:s=\"http://lca.jrc.it/ILCD/Source\" xmlns:u=\"http://lca.jrc.it/ILCD/UnitGroup\" name=\"C2\" scenario=\"Standard scenario\"/>", "<ns11:modules xmlns:ns11=\"http://openlca.org/epd_ilcd\" xmlns=\"http://lca.jrc.it/ILCD/Process\" xmlns:c=\"http://lca.jrc.it/ILCD/Contact\" xmlns:common=\"http://lca.jrc.it/ILCD/Common\" xmlns:epd=\"http://www.iai.kit.edu/EPD/2013\" xmlns:epd2=\"http://www.indata.network/EPD/2019\" xmlns:f=\"http://lca.jrc.it/ILCD/Flow\" xmlns:fp=\"http://lca.jrc.it/ILCD/FlowProperty\" xmlns:m=\"http://lca.jrc.it/ILCD/LCIAMethod\" xmlns:ns9=\"http://www.okworx.com/ILCD/Extensions/2018/Profile\" xmlns:s=\"http://lca.jrc.it/ILCD/Source\" xmlns:u=\"http://lca.jrc.it/ILCD/UnitGroup\" name=\"C3\" scenario=\"Standard scenario\"/>", "<ns11:modules xmlns:ns11=\"http://openlca.org/epd_ilcd\" xmlns=\"http://lca.jrc.it/ILCD/Process\" xmlns:c=\"http://lca.jrc.it/ILCD/Contact\" xmlns:common=\"http://lca.jrc.it/ILCD/Common\" xmlns:epd=\"http://www.iai.kit.edu/EPD/2013\" xmlns:epd2=\"http://www.indata.network/EPD/2019\" xmlns:f=\"http://lca.jrc.it/ILCD/Flow\" xmlns:fp=\"http://lca.jrc.it/ILCD/FlowProperty\" xmlns:m=\"http://lca.jrc.it/ILCD/LCIAMethod\" xmlns:ns9=\"http://www.okworx.com/ILCD/Extensions/2018/Profile\" xmlns:s=\"http://lca.jrc.it/ILCD/Source\" xmlns:u=\"http://lca.jrc.it/ILCD/UnitGroup\" name=\"C4\" scenario=\"Standard scenario\"/>", "<ns11:modules xmlns:ns11=\"http://openlca.org/epd_ilcd\" xmlns=\"http://lca.jrc.it/ILCD/Process\" xmlns:c=\"http://lca.jrc.it/ILCD/Contact\" xmlns:common=\"http://lca.jrc.it/ILCD/Common\" xmlns:epd=\"http://www.iai.kit.edu/EPD/2013\" xmlns:epd2=\"http://www.indata.network/EPD/2019\" xmlns:f=\"http://lca.jrc.it/ILCD/Flow\" xmlns:fp=\"http://lca.jrc.it/ILCD/FlowProperty\" xmlns:m=\"http://lca.jrc.it/ILCD/LCIAMethod\" xmlns:ns9=\"http://www.okworx.com/ILCD/Extensions/2018/Profile\" xmlns:s=\"http://lca.jrc.it/ILCD/Source\" xmlns:u=\"http://lca.jrc.it/ILCD/UnitGroup\" name=\"D\" scenario=\"Standard scenario\"/>"]}}, "quantitativeReference": {"referenceToReferenceFlow": [1], "type": "Reference flow(s)"}, "time": {"referenceYear": 2021, "dataSetValidUntil": 2028, "timeRepresentativenessDescription": [{"value": "The year 2021 represents the time reference for raw materials and electricity consumption.", "lang": "en"}], "other": {"anies": [{"name": "publicationDateOfEPD", "value": 1691020800000}]}}, "geography": {"locationOfOperationSupplyOrProduction": {"descriptionOfRestrictions": [{"value": "Due to manufacturing locations, the exact geographical reference area is Germany, but the present EPD can also be considered representative for the reference area Europe.", "lang": "en"}], "location": "RER"}}, "technology": {"technologyDescriptionAndIncludedProcesses": [{"value": "Schiedel SIH Parat consists of three system components: fireclay inner tube, mineral wool insulation and a lightweight concrete outer wall element. It is available as a single or double duct and with or without ventilation/installation. Each variant is available with different diameters of the exhaust pipe(s). It is suitable for both, gaseous and liquid fuels. The products are resistant to installation damage and chemical and biological long-term degradation. Within this EPD SIH Parat single duct without ventilation/installation based on 4,7 m chimney length and 18 cm diameter was examined. The manufacturing takes place at two different production locations. Outer wall elements production and assembly are caried out at the production location at Schiedel GmbH & Co. KG, Am Wachhübel 2, 04668 Grimma, whereas the ceramic pipe is produced at Schiedel GmbH & Co. KG, Hauptstraße 66, 95676 Wiesau. The Schiedel SIH Parat consists of the outer wall element, ceramic pipe and insulation. At first, outer wall element is produced via mixing of relevant raw materials with subsequent hardening. Manufactured outer wall elements are then transported to Grimma for assembly. Clay and fireclay for the ceramic pipe are first milled, then mixed and pressed into a pipe shape. Subsequently, the pipes are dried and burned. The production of the clay pipe is situated in Wiesau. Eventually, the product is insulated and assembled in Grimma.", "lang": "en"}, {"value": "Der Schiedel SIH Parat besteht aus drei Systemkomponenten: einem Schamotterohr als Innenrohr, einer Wärmedämmung aus Mineralwolle und einem Außenwandelement aus Leichtbeton. Er ist als einzügige oder zweizügige Variante und wahlweise mit oder ohne Lüftungs- bzw. Installationsschacht erhältlich. Jede Variante ist in unterschiedlichen Durchmessern der Abgasleitung(en) verfügbar. Das System ist für gasförmige und flüssige Brennstoffe geeignet. Die Produkte sind widerstandsfähig gegenüber Einbauschäden sowie chemischer und biologischer Langzeitbeanspruchung.\n\nIm Rahmen dieser Umweltproduktdeklaration wurde der SIH Parat in der einzügigen Ausführung ohne Lüftungs- bzw. Installationsschacht auf Basis einer Schornsteinhöhe von 4,7 Metern und einem Durchmesser von 18 Zentimetern untersucht.\n\nDie Herstellung erfolgt an zwei verschiedenen Produktionsstandorten. Die Produktion der Außenwandelemente sowie die Endmontage erfolgen am Standort der Schiedel GmbH & Co. KG in Grimma. Die keramischen Rohre werden am Standort der Schiedel GmbH & Co. KG in Wiesau gefertigt. Der Schiedel SIH Parat setzt sich aus dem Außenwandelement, dem keramischen Rohr und der Dämmung zusammen. Zunächst wird das Außenwandelement durch das Mischen der entsprechenden Rohstoffe mit anschließender Aushärtung hergestellt. Die fertigen Außenwandelemente werden anschließend nach Grimma transportiert. Ton und Schamotte für das keramische Rohr werden zunächst gemahlen, anschließend gemischt und in Rohrform gepresst. Danach erfolgt das Trocknen und Brennen der Rohre. Die Produktion der keramischen Rohre findet in Wiesau statt. Abschließend wird das Produkt in Grimma gedämmt und montiert.", "lang": "de"}], "technologicalApplicability": [{"value": "Schiedel SIH Parat is intended for domestic use as an exhaust system. Prefabricated chimney parts are mainly installed in new buildings and connected to an oven. Installation shall be carried out in accordance with the instructions provided by the manufacturer.", "lang": "en"}, {"value": "Der Schiedel SIH Parat ist für den häuslichen Einsatz als Abgassystem vorgesehen. Die vorgefertigten Schornsteinteile werden hauptsächlich in Neubauten installiert und an einen Ofen angeschlossen. Die Installation ist gemäß den Anweisungen des Herstellers durchzuführen.", "lang": "de"}], "referenceToTechnologyFlowDiagrammOrPicture": [{"shortDescription": [{"value": "Flow Chart for Schiedel SIH Parat", "lang": "en"}], "type": "source data set", "refObjectId": "aeecff84-9af1-4659-8037-c7d10fc6e1dd", "version": "00.00.002"}]}}, "modellingAndValidation": {"LCIMethodAndAllocation": {"typeOfDataSet": "EPD", "other": {"anies": [{"name": "subType", "value": "specific dataset"}]}}, "dataSourcesTreatmentAndRepresentativeness": {"referenceToDataSource": [{"shortDescription": [{"value": "ecoinvent database (general)", "lang": "en"}], "type": "source data set", "refObjectId": "b497a91f-e14b-4b69-8f28-f50eb1576766", "version": "00.03.002"}, {"shortDescription": [{"value": "ecoinvent 3.6 database", "lang": "en"}], "type": "source data set", "refObjectId": "766b9973-5ee8-48a2-8098-72c8e20b369f", "version": "00.00.001"}], "useAdviceForDataSet": [{"value": "Schiedel SIH Parat is intended for domestic use as an exhaust system. Prefabricated chimney parts are mainly installed in new buildings and connected to an oven. Installation shall be carried out in accordance with the instructions provided by the manufacturer.", "lang": "en"}], "other": {"anies": [{"name": "referenceToOriginalEPD", "value": {"shortDescription": {"value": "EPD for Schiedel SIH Parat", "defaultValue": "EPD for Schiedel SIH Parat", "lstrings": [{"lang": "en", "value": "EPD for Schiedel SIH Parat"}]}, "version": {"version": 1, "majorVersion": 0, "minorVersion": 0, "subMinorVersion": 1, "zero": false, "versionString": "00.00.001"}, "type": "source data set", "uuid": {"uuid": "1d2c4ed1-2844-46a7-b7c1-7564c2c72d16"}, "refObjectId": "1d2c4ed1-2844-46a7-b7c1-7564c2c72d16", "versionAsString": "00.00.001", "resourceURLs": ["https://oekobaudat.de/OEKOBAU.DAT/resource/sources/1d2c4ed1-2844-46a7-b7c1-7564c2c72d16/EPD-schiedel-286-en SIH PARAT.pdf?version=00.00.001"]}}]}}, "validation": {"review": [{"reviewDetails": [{"value": "Independent verification of the declaration and data according to ISO 14025:2006.", "lang": "en"}], "referenceToNameOfReviewerAndInstitution": [{"shortDescription": [{"value": "Elisabet Amat - Greenize Projects S.L.U. (Third party verifier)", "lang": "en"}], "type": "contact data set", "refObjectId": "4e247249-fdb4-4f3c-a0fd-b3d3d187667f", "version": "00.00.001"}], "type": "Independent external review"}]}, "complianceDeclarations": {"compliance": [{"referenceToComplianceSystem": {"shortDescription": [{"value": "EN 15804+A2 (EF 3.0)", "lang": "de"}, {"value": "EN 15804+A2 (EF 3.0)", "lang": "en"}], "type": "source data set", "refObjectId": "c0016b33-8cf7-415c-ac6e-deba0d21440d", "version": "00.02.000"}}, {"referenceToComplianceSystem": {"shortDescription": [{"value": "ISO 14025", "lang": "en"}], "type": "source data set", "refObjectId": "4f2eb655-6e44-4874-a95a-e28f5442cd4d", "version": "00.00.001"}}]}}, "administrativeInformation": {"commissionerAndGoal": {"referenceToCommissioner": [{"shortDescription": [{"value": "Schiedel GmbH & Co. KG", "lang": "en"}], "type": "contact data set", "refObjectId": "91ff6c83-bb9c-40c7-b627-f11d3a92afc4", "version": "00.00.001"}]}, "dataGenerator": {"referenceToPersonOrEntityGeneratingTheDataSet": [{"shortDescription": [{"value": "Kiwa GmbH (Berlin)", "lang": "en"}], "type": "contact data set", "refObjectId": "3ea4a87a-3f88-4633-b7e7-1bbdd272be43", "version": "00.00.002"}]}, "dataEntryBy": {"timeStamp": 1761817157147, "referenceToDataSetFormat": [{"shortDescription": [{"value": "ILCD format", "lang": "en"}], "type": "source data set", "refObjectId": "a97a0155-0234-4b87-b4ce-a45da52f2a40", "version": "01.00.000", "uri": "http://lca.jrc.ec.europa.eu/lcainfohub/sample_data/ilcd/sources/ILCD_Format_a97a0155-0234-4b87-b4ce-a45da52f2a40_01.00.000.xml"}, {"shortDescription": [{"value": "EPD Data Format Extensions v1.2", "lang": "en"}, {"value": "EPD-Datenformaterweiterungen v1.2", "lang": "de"}], "type": "source data set", "refObjectId": "a29449fd-aa2f-4de8-b5d7-4b06b43c6fde", "version": "00.01.000"}], "referenceToPersonOrEntityEnteringTheData": {"shortDescription": [{"value": "Kiwa-Ecobility Experts, Kiwa GmbH (Berlin)", "lang": "en"}], "type": "contact data set", "refObjectId": "eb52a9a8-9d0f-40ce-a5c9-7b78f5615e5a", "version": "00.00.002"}}, "publicationAndOwnership": {"dataSetVersion": "00.00.012", "referenceToRegistrationAuthority": {"shortDescription": [{"value": "Kiwa-Ecobility Experts, Kiwa GmbH (Berlin)", "lang": "en"}], "type": "contact data set", "refObjectId": "eb52a9a8-9d0f-40ce-a5c9-7b78f5615e5a", "version": "00.00.002"}, "registrationNumber": "EPD-Schiedel-286-EN", "referenceToOwnershipOfDataSet": {"shortDescription": [{"value": "Schiedel GmbH & Co. KG", "lang": "en"}], "type": "contact data set", "refObjectId": "91ff6c83-bb9c-40c7-b627-f11d3a92afc4", "version": "00.00.001"}, "copyright": true, "licenseType": "Free of charge for all users and uses", "accessRestrictions": [{"value": "None", "lang": "en"}], "other": {"anies": [{"name": "referenceToPublisher", "value": {"shortDescription": [{"value": "Kiwa-Ecobility Experts, Kiwa GmbH (Berlin)", "lang": "en"}], "type": "contact data set", "refObjectId": "eb52a9a8-9d0f-40ce-a5c9-7b78f5615e5a", "version": "00.00.002"}}]}}}, "exchanges": {"exchange": [{"dataSetInternalID": 1, "referenceToFlowDataSet": {"shortDescription": [{"value": "Schiedel SIH Parat", "lang": "en"}], "type": "flow data set", "refObjectId": "27c58e4c-9694-4ed7-aa39-0866d7abf787", "version": "00.00.005"}, "meanAmount": 1.0, "resultingAmount": 1.0, "referenceFlow": true, "resultingflowAmount": 1.0, "flowProperties": [{"name": [{"lang": "en", "value": "Mass"}, {"lang": "de", "value": "Masse"}], "uuid": "93a60a56-a3c8-11da-a746-0800200b9a66", "referenceFlowProperty": true, "meanValue": 1.0, "referenceUnit": "kg", "unitGroupUUID": "ad38d542-3fe9-439d-9b95-2f5f7752acaf"}, {"name": [{"lang": "de", "value": "Länge"}, {"lang": "en", "value": "Length"}], "uuid": "838aaa23-0117-11db-92e3-0800200c9a66", "meanValue": 0.00812}], "materialProperties": [{"name": "linear density", "value": "123.15", "unit": "kg/m"}], "typeOfFlow": "Product flow", "classification": {"classHierarchy": "Komponenten von Fenstern und Vorhangfassaden / Tageslichtsysteme und Rauch- / Wärmeabzugsanlagen  / Rauch-/Wärmeabzugsanlagen", "name": "OEKOBAU.DAT"}}, {"dataSetInternalID": 2, "referenceToFlowDataSet": {"shortDescription": [{"value": "Components for re-use (CRU)", "lang": "en"}, {"value": "Komponenten für die Wiederverwendung (CRU)", "lang": "de"}, {"value": "Componentes para su reutilización (CRU)", "lang": "es"}], "type": "flow data set", "refObjectId": "a2b32f97-3fc7-4af2-b209-525bc6426f33", "version": "30.00.000", "uri": "../flows/a2b32f97-3fc7-4af2-b209-525bc6426f33.xml"}, "exchange direction": "OUTPUT", "meanAmount": 0.0, "other": {"anies": [{"value": "0.0", "module": "A1", "scenario": "Standard scenario"}, {"value": "0.0", "module": "A2", "scenario": "Standard scenario"}, {"value": "0.0", "module": "A3", "scenario": "Standard scenario"}, {"value": "0.0", "module": "C1", "scenario": "Standard scenario"}, {"value": "0.0", "module": "C2", "scenario": "Standard scenario"}, {"value": "0.0", "module": "C3", "scenario": "Standard scenario"}, {"value": "0.0", "module": "C4", "scenario": "Standard scenario"}, {"value": "0.0", "module": "D", "scenario": "Standard scenario"}, {"name": "referenceToUnitGroupDataSet", "value": {"shortDescription": [{"value": "kg", "lang": "en"}], "type": "unit group data set", "refObjectId": "ad38d542-3fe9-439d-9b95-2f5f7752acaf", "version": "30.00.000", "uri": "../unitgroups/ad38d542-3fe9-439d-9b95-2f5f7752acaf.xml"}}]}, "flowProperties": [], "typeOfFlow": "Other flow", "classification": {"classHierarchy": "Größen / Umweltliche Größen / EPD EN 15804 / LCI Indikatoren", "name": "GaBiCategories"}}, {"dataSetInternalID": 3, "referenceToFlowDataSet": {"shortDescription": [{"value": "Exported electrical energy (EEE)", "lang": "en"}, {"value": "Exportierte elektrische Energie (EEE)", "lang": "de"}, {"value": "Energía exportada electrica (EEE)", "lang": "es"}], "type": "flow data set", "refObjectId": "4da0c987-2b76-40d6-9e9e-82a017aaaf29", "version": "30.00.000", "uri": "../flows/4da0c987-2b76-40d6-9e9e-82a017aaaf29.xml"}, "exchange direction": "OUTPUT", "meanAmount": 0.0, "other": {"anies": [{"value": "0.0", "module": "A1", "scenario": "Standard scenario"}, {"value": "0.0", "module": "A2", "scenario": "Standard scenario"}, {"value": "0.0", "module": "A3", "scenario": "Standard scenario"}, {"value": "0.0", "module": "C1", "scenario": "Standard scenario"}, {"value": "0.0", "module": "C2", "scenario": "Standard scenario"}, {"value": "0.0", "module": "C3", "scenario": "Standard scenario"}, {"value": "0.0", "module": "C4", "scenario": "Standard scenario"}, {"value": "0.0", "module": "D", "scenario": "Standard scenario"}, {"name": "referenceToUnitGroupDataSet", "value": {"shortDescription": [{"value": "MJ", "lang": "en"}], "type": "unit group data set", "refObjectId": "93a60a57-a3c8-11da-a746-0800200c9a66", "version": "03.00.000", "uri": "../unitgroups/93a60a57-a3c8-11da-a746-0800200c9a66.xml"}}]}, "flowProperties": [], "typeOfFlow": "Other flow", "classification": {"classHierarchy": "Größen / Umweltliche Größen / EPD EN 15804 / LCI Indikatoren", "name": "GaBiCategories"}}, {"dataSetInternalID": 4, "referenceToFlowDataSet": {"shortDescription": [{"value": "Exported thermal energy (EET)", "lang": "en"}, {"value": "Exportierte thermische Energie (EET)", "lang": "de"}, {"value": "Energía exportada termal (EET)", "lang": "es"}], "type": "flow data set", "refObjectId": "98daf38a-7a79-46d3-9a37-2b7bd0955810", "version": "30.00.000", "uri": "../flows/98daf38a-7a79-46d3-9a37-2b7bd0955810.xml"}, "exchange direction": "OUTPUT", "meanAmount": 0.0, "other": {"anies": [{"value": "0.0", "module": "A1", "scenario": "Standard scenario"}, {"value": "0.0", "module": "A2", "scenario": "Standard scenario"}, {"value": "0.0", "module": "A3", "scenario": "Standard scenario"}, {"value": "0.0", "module": "C1", "scenario": "Standard scenario"}, {"value": "0.0", "module": "C2", "scenario": "Standard scenario"}, {"value": "0.0", "module": "C3", "scenario": "Standard scenario"}, {"value": "0.0", "module": "C4", "scenario": "Standard scenario"}, {"value": "0.0", "module": "D", "scenario": "Standard scenario"}, {"name": "referenceToUnitGroupDataSet", "value": {"shortDescription": [{"value": "MJ", "lang": "en"}], "type": "unit group data set", "refObjectId": "93a60a57-a3c8-11da-a746-0800200c9a66", "version": "03.00.000", "uri": "../unitgroups/93a60a57-a3c8-11da-a746-0800200c9a66.xml"}}]}, "flowProperties": [], "typeOfFlow": "Other flow", "classification": {"classHierarchy": "Größen / Umweltliche Größen / EPD EN 15804 / LCI Indikatoren", "name": "GaBiCategories"}}, {"dataSetInternalID": 5, "referenceToFlowDataSet": {"shortDescription": [{"value": "Hazardous waste disposed (HWD)", "lang": "en"}, {"value": "Gefährlicher Abfall zur Deponie (HWD)", "lang": "de"}, {"value": "Residuos peligrosos eliminados (HWD)", "lang": "es"}], "type": "flow data set", "refObjectId": "430f9e0f-59b2-46a0-8e0d-55e0e84948fc", "version": "30.00.000", "uri": "../flows/430f9e0f-59b2-46a0-8e0d-55e0e84948fc.xml"}, "exchange direction": "OUTPUT", "meanAmount": 0.0, "other": {"anies": [{"value": "1.09E-4", "module": "A1", "scenario": "Standard scenario"}, {"value": "2.07E-6", "module": "A2", "scenario": "Standard scenario"}, {"value": "4.79E-6", "module": "A3", "scenario": "Standard scenario"}, {"value": "1.32E-6", "module": "C1", "scenario": "Standard scenario"}, {"value": "3.06E-7", "module": "C2", "scenario": "Standard scenario"}, {"value": "3.19E-8", "module": "C3", "scenario": "Standard scenario"}, {"value": "3.8E-8", "module": "C4", "scenario": "Standard scenario"}, {"value": "-8.88E-8", "module": "D", "scenario": "Standard scenario"}, {"name": "referenceToUnitGroupDataSet", "value": {"shortDescription": [{"value": "kg", "lang": "en"}], "type": "unit group data set", "refObjectId": "ad38d542-3fe9-439d-9b95-2f5f7752acaf", "version": "30.00.000", "uri": "../unitgroups/ad38d542-3fe9-439d-9b95-2f5f7752acaf.xml"}}]}, "flowProperties": [], "typeOfFlow": "Other flow", "classification": {"classHierarchy": "Größen / Umweltliche Größen / EPD EN 15804 / LCI Indikatoren", "name": "GaBiCategories"}}, {"dataSetInternalID": 6, "referenceToFlowDataSet": {"shortDescription": [{"value": "Materials for energy recovery (MER)", "lang": "en"}, {"value": "Stoffe für die Energierückgewinnung (MER)", "lang": "de"}, {"value": "Materiales para valorización energética (recuperación de energía) (MER)", "lang": "es"}], "type": "flow data set", "refObjectId": "59a9181c-3aaf-46ee-8b13-2b3723b6e447", "version": "30.00.000", "uri": "../flows/59a9181c-3aaf-46ee-8b13-2b3723b6e447.xml"}, "exchange direction": "OUTPUT", "meanAmount": 0.0, "other": {"anies": [{"value": "0.0", "module": "A1", "scenario": "Standard scenario"}, {"value": "0.0", "module": "A2", "scenario": "Standard scenario"}, {"value": "0.0", "module": "A3", "scenario": "Standard scenario"}, {"value": "0.0", "module": "C1", "scenario": "Standard scenario"}, {"value": "0.0", "module": "C2", "scenario": "Standard scenario"}, {"value": "0.0", "module": "C3", "scenario": "Standard scenario"}, {"value": "0.0", "module": "C4", "scenario": "Standard scenario"}, {"value": "0.0", "module": "D", "scenario": "Standard scenario"}, {"name": "referenceToUnitGroupDataSet", "value": {"shortDescription": [{"value": "kg", "lang": "en"}], "type": "unit group data set", "refObjectId": "ad38d542-3fe9-439d-9b95-2f5f7752acaf", "version": "30.00.000", "uri": "../unitgroups/ad38d542-3fe9-439d-9b95-2f5f7752acaf.xml"}}]}, "flowProperties": [], "typeOfFlow": "Other flow", "classification": {"classHierarchy": "Größen / Umweltliche Größen / EPD EN 15804 / LCI Indikatoren", "name": "GaBiCategories"}}, {"dataSetInternalID": 7, "referenceToFlowDataSet": {"shortDescription": [{"value": "Materials for recycling (MFR)", "lang": "en"}, {"value": "Stoffe zum Recycling (MFR)", "lang": "de"}, {"value": "Materiales para el reciclaje (MFR)", "lang": "es"}], "type": "flow data set", "refObjectId": "d7fe48a5-4103-49c8-9aae-b0b5dfdbd6ae", "version": "30.00.000", "uri": "../flows/d7fe48a5-4103-49c8-9aae-b0b5dfdbd6ae.xml"}, "exchange direction": "OUTPUT", "meanAmount": 0.0, "other": {"anies": [{"value": "0.0", "module": "A1", "scenario": "Standard scenario"}, {"value": "0.0", "module": "A2", "scenario": "Standard scenario"}, {"value": "0.0922", "module": "A3", "scenario": "Standard scenario"}, {"value": "0.0", "module": "C1", "scenario": "Standard scenario"}, {"value": "0.0", "module": "C2", "scenario": "Standard scenario"}, {"value": "0.839", "module": "C3", "scenario": "Standard scenario"}, {"value": "0.0", "module": "C4", "scenario": "Standard scenario"}, {"value": "0.0", "module": "D", "scenario": "Standard scenario"}, {"name": "referenceToUnitGroupDataSet", "value": {"shortDescription": [{"value": "kg", "lang": "en"}], "type": "unit group data set", "refObjectId": "ad38d542-3fe9-439d-9b95-2f5f7752acaf", "version": "30.00.000", "uri": "../unitgroups/ad38d542-3fe9-439d-9b95-2f5f7752acaf.xml"}}]}, "flowProperties": [], "typeOfFlow": "Other flow", "classification": {"classHierarchy": "Größen / Umweltliche Größen / EPD EN 15804 / LCI Indikatoren", "name": "GaBiCategories"}}, {"dataSetInternalID": 8, "referenceToFlowDataSet": {"shortDescription": [{"value": "Use of net fresh water (FW)", "lang": "en"}, {"value": "Einsatz von Süßwasserressourcen (FW)", "lang": "de"}, {"value": "Uso neto de recursos de agua dulce (FW)", "lang": "es"}], "type": "flow data set", "refObjectId": "3cf952c8-f3a4-461d-8c96-96456ca62246", "version": "30.00.000", "uri": "../flows/3cf952c8-f3a4-461d-8c96-96456ca62246.xml"}, "exchange direction": "INPUT", "meanAmount": 0.0, "other": {"anies": [{"value": "0.00173", "module": "A1", "scenario": "Standard scenario"}, {"value": "9.96E-5", "module": "A2", "scenario": "Standard scenario"}, {"value": "4.68E-4", "module": "A3", "scenario": "Standard scenario"}, {"value": "2.5E-5", "module": "C1", "scenario": "Standard scenario"}, {"value": "1.47E-5", "module": "C2", "scenario": "Standard scenario"}, {"value": "6.13E-6", "module": "C3", "scenario": "Standard scenario"}, {"value": "2.71E-5", "module": "C4", "scenario": "Standard scenario"}, {"value": "-0.00118", "module": "D", "scenario": "Standard scenario"}, {"name": "referenceToUnitGroupDataSet", "value": {"shortDescription": [{"value": "m3", "lang": "en"}], "type": "unit group data set", "refObjectId": "cd950537-0a98-4044-9ba7-9f9a68d0a504", "version": "30.00.000", "uri": "../unitgroups/cd950537-0a98-4044-9ba7-9f9a68d0a504.xml"}}]}, "flowProperties": [], "typeOfFlow": "Other flow", "classification": {"classHierarchy": "Größen / Umweltliche Größen / EPD EN 15804 / LCI Indikatoren", "name": "GaBiCategories"}}, {"dataSetInternalID": 9, "referenceToFlowDataSet": {"shortDescription": [{"value": "Non-hazardous waste disposed (NHWD)", "lang": "en"}, {"value": "Entsorgter nicht gefährlicher Abfall (NHWD)", "lang": "de"}, {"value": "Residuos no peligrosos eliminados (NHWD)", "lang": "es"}], "type": "flow data set", "refObjectId": "b29ef66b-e286-4afa-949f-62f1a7b4d7fa", "version": "30.00.000", "uri": "../flows/b29ef66b-e286-4afa-949f-62f1a7b4d7fa.xml"}, "exchange direction": "OUTPUT", "meanAmount": 0.0, "other": {"anies": [{"value": "0.0156", "module": "A1", "scenario": "Standard scenario"}, {"value": "0.0519", "module": "A2", "scenario": "Standard scenario"}, {"value": "0.0155", "module": "A3", "scenario": "Standard scenario"}, {"value": "5.75E-4", "module": "C1", "scenario": "Standard scenario"}, {"value": "0.00765", "module": "C2", "scenario": "Standard scenario"}, {"value": "0.00256", "module": "C3", "scenario": "Standard scenario"}, {"value": "0.173", "module": "C4", "scenario": "Standard scenario"}, {"value": "-4.76E-4", "module": "D", "scenario": "Standard scenario"}, {"name": "referenceToUnitGroupDataSet", "value": {"shortDescription": [{"value": "kg", "lang": "en"}], "type": "unit group data set", "refObjectId": "ad38d542-3fe9-439d-9b95-2f5f7752acaf", "version": "30.00.000", "uri": "../unitgroups/ad38d542-3fe9-439d-9b95-2f5f7752acaf.xml"}}]}, "flowProperties": [], "typeOfFlow": "Other flow", "classification": {"classHierarchy": "Größen / Umweltliche Größen / EPD EN 15804 / LCI Indikatoren", "name": "GaBiCategories"}}, {"dataSetInternalID": 10, "referenceToFlowDataSet": {"shortDescription": [{"value": "Use of non renewable primary energy (PENRE)", "lang": "en"}, {"value": "Nicht-erneuerbare Primärenergie als Energieträger (PENRE)", "lang": "de"}, {"value": "Uso de energía primaria no renovable, excluyendo los recursos de energía primaria no renovable utilizada como materia prima (PENRE)", "lang": "es"}], "type": "flow data set", "refObjectId": "ac857178-2b45-46ec-892a-a9a4332f0372", "version": "38.00.000", "uri": "../flows/ac857178-2b45-46ec-892a-a9a4332f0372.xml"}, "exchange direction": "INPUT", "meanAmount": 0.0, "other": {"anies": [{"value": "2.34", "module": "A1", "scenario": "Standard scenario"}, {"value": "0.868", "module": "A2", "scenario": "Standard scenario"}, {"value": "1.4", "module": "A3", "scenario": "Standard scenario"}, {"value": "0.516", "module": "C1", "scenario": "Standard scenario"}, {"value": "0.128", "module": "C2", "scenario": "Standard scenario"}, {"value": "0.0196", "module": "C3", "scenario": "Standard scenario"}, {"value": "0.027", "module": "C4", "scenario": "Standard scenario"}, {"value": "-0.0466", "module": "D", "scenario": "Standard scenario"}, {"name": "referenceToUnitGroupDataSet", "value": {"shortDescription": [{"value": "MJ", "lang": "en"}], "type": "unit group data set", "refObjectId": "93a60a57-a3c8-11da-a746-0800200c9a66", "version": "03.00.000", "uri": "../unitgroups/93a60a57-a3c8-11da-a746-0800200c9a66.xml"}}]}, "flowProperties": [], "typeOfFlow": "Other flow", "classification": {"classHierarchy": "Quantities", "name": "GaBiCategories"}}, {"dataSetInternalID": 11, "referenceToFlowDataSet": {"shortDescription": [{"value": "Use of non renewable primary energy resources used as raw materials (PENRM)", "lang": "en"}, {"value": "Nicht-erneuerbare Primärenergie zur stofflichen Nutzung (PENRM)", "lang": "de"}, {"value": "Uso de la energía primaria no renovable utilizada como materia prima (PENRM)", "lang": "es"}], "type": "flow data set", "refObjectId": "1421caa0-679d-4bf4-b282-0eb850ccae27", "version": "38.00.000", "uri": "../flows/1421caa0-679d-4bf4-b282-0eb850ccae27.xml"}, "exchange direction": "INPUT", "meanAmount": 0.0, "other": {"anies": [{"value": "0.00702", "module": "A1", "scenario": "Standard scenario"}, {"value": "0.0", "module": "A2", "scenario": "Standard scenario"}, {"value": "7.71E-4", "module": "A3", "scenario": "Standard scenario"}, {"value": "0.0", "module": "C1", "scenario": "Standard scenario"}, {"value": "0.0", "module": "C2", "scenario": "Standard scenario"}, {"value": "0.0", "module": "C3", "scenario": "Standard scenario"}, {"value": "0.0", "module": "C4", "scenario": "Standard scenario"}, {"value": "0.0", "module": "D", "scenario": "Standard scenario"}, {"name": "referenceToUnitGroupDataSet", "value": {"shortDescription": [{"value": "MJ", "lang": "en"}], "type": "unit group data set", "refObjectId": "93a60a57-a3c8-11da-a746-0800200c9a66", "version": "03.00.000", "uri": "../unitgroups/93a60a57-a3c8-11da-a746-0800200c9a66.xml"}}]}, "flowProperties": [], "typeOfFlow": "Other flow", "classification": {"classHierarchy": "Quantities", "name": "GaBiCategories"}}, {"dataSetInternalID": 12, "referenceToFlowDataSet": {"shortDescription": [{"value": "Use of non renewable secondary fuels (NRSF)", "lang": "en"}, {"value": "Nicht erneuerbare Sekundärbrennstoffe (NRSF)", "lang": "de"}, {"value": "Uso de combustibles secundarios no renovables (NRSF)", "lang": "es"}], "type": "flow data set", "refObjectId": "89def144-d39a-4287-b86f-efde453ddcb2", "version": "30.00.000", "uri": "../flows/89def144-d39a-4287-b86f-efde453ddcb2.xml"}, "exchange direction": "INPUT", "meanAmount": 0.0, "other": {"anies": [{"value": "2.45E-4", "module": "A1", "scenario": "Standard scenario"}, {"value": "0.0", "module": "A2", "scenario": "Standard scenario"}, {"value": "7.34E-6", "module": "A3", "scenario": "Standard scenario"}, {"value": "0.0", "module": "C1", "scenario": "Standard scenario"}, {"value": "0.0", "module": "C2", "scenario": "Standard scenario"}, {"value": "0.0", "module": "C3", "scenario": "Standard scenario"}, {"value": "0.0", "module": "C4", "scenario": "Standard scenario"}, {"value": "0.0", "module": "D", "scenario": "Standard scenario"}, {"name": "referenceToUnitGroupDataSet", "value": {"shortDescription": [{"value": "MJ", "lang": "en"}], "type": "unit group data set", "refObjectId": "93a60a57-a3c8-11da-a746-0800200c9a66", "version": "03.00.000", "uri": "../unitgroups/93a60a57-a3c8-11da-a746-0800200c9a66.xml"}}]}, "flowProperties": [], "typeOfFlow": "Other flow", "classification": {"classHierarchy": "Größen / Umweltliche Größen / EPD EN 15804 / LCI Indikatoren", "name": "GaBiCategories"}}, {"dataSetInternalID": 13, "referenceToFlowDataSet": {"shortDescription": [{"value": "Radioactive waste disposed (RWD)", "lang": "en"}, {"value": "Entsorgter radioaktiver Abfall (RWD)", "lang": "de"}, {"value": "Residuos radiactivos eliminados (RWD)", "lang": "es"}], "type": "flow data set", "refObjectId": "3449546e-52ad-4b39-b809-9fb77cea8ff6", "version": "30.00.000", "uri": "../flows/3449546e-52ad-4b39-b809-9fb77cea8ff6.xml"}, "exchange direction": "OUTPUT", "meanAmount": 0.0, "other": {"anies": [{"value": "7.99E-6", "module": "A1", "scenario": "Standard scenario"}, {"value": "5.37E-6", "module": "A2", "scenario": "Standard scenario"}, {"value": "4.51E-6", "module": "A3", "scenario": "Standard scenario"}, {"value": "3.37E-6", "module": "C1", "scenario": "Standard scenario"}, {"value": "7.92E-7", "module": "C2", "scenario": "Standard scenario"}, {"value": "8.24E-8", "module": "C3", "scenario": "Standard scenario"}, {"value": "1.67E-7", "module": "C4", "scenario": "Standard scenario"}, {"value": "-1.92E-7", "module": "D", "scenario": "Standard scenario"}, {"name": "referenceToUnitGroupDataSet", "value": {"shortDescription": [{"value": "kg", "lang": "en"}], "type": "unit group data set", "refObjectId": "ad38d542-3fe9-439d-9b95-2f5f7752acaf", "version": "30.00.000", "uri": "../unitgroups/ad38d542-3fe9-439d-9b95-2f5f7752acaf.xml"}}]}, "flowProperties": [], "typeOfFlow": "Other flow", "classification": {"classHierarchy": "Größen / Umweltliche Größen / EPD EN 15804 / LCI Indikatoren", "name": "GaBiCategories"}}, {"dataSetInternalID": 14, "referenceToFlowDataSet": {"shortDescription": [{"value": "Use of renewable primary energy (PERE)", "lang": "en"}, {"value": "Erneuerbare Primärenergie als Energieträger (PERE)", "lang": "de"}, {"value": "Uso de energía primaria renovable excluyendo los recursos de energía primaria renovable utilizada como materia prima (PERE)", "lang": "es"}], "type": "flow data set", "refObjectId": "20f32be5-0398-4288-9b6d-accddd195317", "version": "38.00.000", "uri": "../flows/20f32be5-0398-4288-9b6d-accddd195317.xml"}, "exchange direction": "INPUT", "meanAmount": 0.0, "other": {"anies": [{"value": "0.297", "module": "A1", "scenario": "Standard scenario"}, {"value": "0.0102", "module": "A2", "scenario": "Standard scenario"}, {"value": "0.271", "module": "A3", "scenario": "Standard scenario"}, {"value": "0.00263", "module": "C1", "scenario": "Standard scenario"}, {"value": "0.00151", "module": "C2", "scenario": "Standard scenario"}, {"value": "0.00104", "module": "C3", "scenario": "Standard scenario"}, {"value": "2.05E-4", "module": "C4", "scenario": "Standard scenario"}, {"value": "-0.00304", "module": "D", "scenario": "Standard scenario"}, {"name": "referenceToUnitGroupDataSet", "value": {"shortDescription": [{"value": "MJ", "lang": "en"}], "type": "unit group data set", "refObjectId": "93a60a57-a3c8-11da-a746-0800200c9a66", "version": "03.00.000", "uri": "../unitgroups/93a60a57-a3c8-11da-a746-0800200c9a66.xml"}}]}, "flowProperties": [], "typeOfFlow": "Other flow", "classification": {"classHierarchy": "Quantities", "name": "GaBiCategories"}}, {"dataSetInternalID": 15, "referenceToFlowDataSet": {"shortDescription": [{"value": "Use of renewable primary energy resources used as raw materials (PERM)", "lang": "en"}, {"value": "Erneuerbare Primärenergie zur stofflichen Nutzung (PERM)", "lang": "de"}, {"value": "Uso de energía primaria renovable utilizada como materia prima (PERM)", "lang": "es"}], "type": "flow data set", "refObjectId": "fb3ec0de-548d-4508-aea5-00b73bf6f702", "version": "38.00.000", "uri": "../flows/fb3ec0de-548d-4508-aea5-00b73bf6f702.xml"}, "exchange direction": "INPUT", "meanAmount": 0.0, "other": {"anies": [{"value": "0.0", "module": "A1", "scenario": "Standard scenario"}, {"value": "0.0", "module": "A2", "scenario": "Standard scenario"}, {"value": "0.0", "module": "A3", "scenario": "Standard scenario"}, {"value": "0.0", "module": "C1", "scenario": "Standard scenario"}, {"value": "0.0", "module": "C2", "scenario": "Standard scenario"}, {"value": "0.0", "module": "C3", "scenario": "Standard scenario"}, {"value": "0.0", "module": "C4", "scenario": "Standard scenario"}, {"value": "0.0", "module": "D", "scenario": "Standard scenario"}, {"name": "referenceToUnitGroupDataSet", "value": {"shortDescription": [{"value": "MJ", "lang": "en"}], "type": "unit group data set", "refObjectId": "93a60a57-a3c8-11da-a746-0800200c9a66", "version": "03.00.000", "uri": "../unitgroups/93a60a57-a3c8-11da-a746-0800200c9a66.xml"}}]}, "flowProperties": [], "typeOfFlow": "Other flow", "classification": {"classHierarchy": "Quantities", "name": "GaBiCategories"}}, {"dataSetInternalID": 16, "referenceToFlowDataSet": {"shortDescription": [{"value": "Use of renewable secondary fuels (RSF)", "lang": "en"}, {"value": "Erneuerbare Sekundärbrennstoffe (RSF)", "lang": "de"}, {"value": "Uso de combustibles secundarios renovables (RSF)", "lang": "es"}], "type": "flow data set", "refObjectId": "64333088-a55f-4aa2-9a31-c10b07816787", "version": "30.00.000", "uri": "../flows/64333088-a55f-4aa2-9a31-c10b07816787.xml"}, "exchange direction": "INPUT", "meanAmount": 0.0, "other": {"anies": [{"value": "1.08E-4", "module": "A1", "scenario": "Standard scenario"}, {"value": "0.0", "module": "A2", "scenario": "Standard scenario"}, {"value": "3.25E-6", "module": "A3", "scenario": "Standard scenario"}, {"value": "0.0", "module": "C1", "scenario": "Standard scenario"}, {"value": "0.0", "module": "C2", "scenario": "Standard scenario"}, {"value": "0.0", "module": "C3", "scenario": "Standard scenario"}, {"value": "0.0", "module": "C4", "scenario": "Standard scenario"}, {"value": "0.0", "module": "D", "scenario": "Standard scenario"}, {"name": "referenceToUnitGroupDataSet", "value": {"shortDescription": [{"value": "MJ", "lang": "en"}], "type": "unit group data set", "refObjectId": "93a60a57-a3c8-11da-a746-0800200c9a66", "version": "03.00.000", "uri": "../unitgroups/93a60a57-a3c8-11da-a746-0800200c9a66.xml"}}]}, "flowProperties": [], "typeOfFlow": "Other flow", "classification": {"classHierarchy": "Größen / Umweltliche Größen / EPD EN 15804 / LCI Indikatoren", "name": "GaBiCategories"}}, {"dataSetInternalID": 17, "referenceToFlowDataSet": {"shortDescription": [{"value": "Use of secondary material (SM)", "lang": "en"}, {"value": "Einsatz von Sekundärstoffen (SM)", "lang": "de"}, {"value": "Uso de materiales secundarios (SM)", "lang": "es"}], "type": "flow data set", "refObjectId": "c6a1f35f-2d09-4f54-8dfb-97e502e1ce92", "version": "30.00.000", "uri": "../flows/c6a1f35f-2d09-4f54-8dfb-97e502e1ce92.xml"}, "exchange direction": "INPUT", "meanAmount": 0.0, "other": {"anies": [{"value": "0.0", "module": "A1", "scenario": "Standard scenario"}, {"value": "0.0", "module": "A2", "scenario": "Standard scenario"}, {"value": "0.0", "module": "A3", "scenario": "Standard scenario"}, {"value": "0.0", "module": "C1", "scenario": "Standard scenario"}, {"value": "0.0", "module": "C2", "scenario": "Standard scenario"}, {"value": "0.0", "module": "C3", "scenario": "Standard scenario"}, {"value": "0.0", "module": "C4", "scenario": "Standard scenario"}, {"value": "0.0", "module": "D", "scenario": "Standard scenario"}, {"name": "referenceToUnitGroupDataSet", "value": {"shortDescription": [{"value": "kg", "lang": "en"}], "type": "unit group data set", "refObjectId": "ad38d542-3fe9-439d-9b95-2f5f7752acaf", "version": "30.00.000", "uri": "../unitgroups/ad38d542-3fe9-439d-9b95-2f5f7752acaf.xml"}}]}, "flowProperties": [], "typeOfFlow": "Other flow", "classification": {"classHierarchy": "Größen / Umweltliche Größen / EPD EN 15804 / LCI Indikatoren", "name": "GaBiCategories"}}, {"dataSetInternalID": 18, "referenceToFlowDataSet": {"shortDescription": [{"value": "Total use of non-renewable primary energy resources (PENRT)", "lang": "en"}, {"value": "Total nicht erneuerbare Primärenergie (PENRT)", "lang": "de"}, {"value": "Uso total de la energía primaria no renovable (energía primaria y recursos de energía primaria renovable utilizada como materia prima) (PENRT)", "lang": "es"}], "type": "flow data set", "refObjectId": "06159210-646b-4c8d-8583-da9b3b95a6c1", "version": "30.00.000", "uri": "../flows/06159210-646b-4c8d-8583-da9b3b95a6c1.xml"}, "exchange direction": "INPUT", "meanAmount": 0.0, "other": {"anies": [{"value": "2.35", "module": "A1", "scenario": "Standard scenario"}, {"value": "0.868", "module": "A2", "scenario": "Standard scenario"}, {"value": "1.4", "module": "A3", "scenario": "Standard scenario"}, {"value": "0.516", "module": "C1", "scenario": "Standard scenario"}, {"value": "0.128", "module": "C2", "scenario": "Standard scenario"}, {"value": "0.0196", "module": "C3", "scenario": "Standard scenario"}, {"value": "0.027", "module": "C4", "scenario": "Standard scenario"}, {"value": "-0.0466", "module": "D", "scenario": "Standard scenario"}, {"name": "referenceToUnitGroupDataSet", "value": {"shortDescription": [{"value": "MJ", "lang": "en"}], "type": "unit group data set", "refObjectId": "93a60a57-a3c8-11da-a746-0800200c9a66", "version": "03.00.000", "uri": "../unitgroups/93a60a57-a3c8-11da-a746-0800200c9a66.xml"}}]}, "flowProperties": [], "typeOfFlow": "Other flow", "classification": {"classHierarchy": "Größen / Umweltliche Größen / EPD EN 15804 / LCI Indikatoren", "name": "GaBiCategories"}}, {"dataSetInternalID": 19, "referenceToFlowDataSet": {"shortDescription": [{"value": "Total use of renewable primary energy resources (PERT)", "lang": "en"}, {"value": "Total erneuerbare Primärenergie (PERT)", "lang": "de"}, {"value": "Uso total de la energía primaria renovable (energía primaria y recursos de energía primaria renovable utilizada como materia prima) (PERT)", "lang": "es"}], "type": "flow data set", "refObjectId": "53f97275-fa8a-4cdd-9024-65936002acd0", "version": "30.00.000", "uri": "../flows/53f97275-fa8a-4cdd-9024-65936002acd0.xml"}, "exchange direction": "INPUT", "meanAmount": 0.0, "other": {"anies": [{"value": "0.297", "module": "A1", "scenario": "Standard scenario"}, {"value": "0.0102", "module": "A2", "scenario": "Standard scenario"}, {"value": "0.271", "module": "A3", "scenario": "Standard scenario"}, {"value": "0.00263", "module": "C1", "scenario": "Standard scenario"}, {"value": "0.00151", "module": "C2", "scenario": "Standard scenario"}, {"value": "0.00104", "module": "C3", "scenario": "Standard scenario"}, {"value": "2.05E-4", "module": "C4", "scenario": "Standard scenario"}, {"value": "-0.00304", "module": "D", "scenario": "Standard scenario"}, {"name": "referenceToUnitGroupDataSet", "value": {"shortDescription": [{"value": "MJ", "lang": "en"}], "type": "unit group data set", "refObjectId": "93a60a57-a3c8-11da-a746-0800200c9a66", "version": "03.00.000", "uri": "../unitgroups/93a60a57-a3c8-11da-a746-0800200c9a66.xml"}}]}, "flowProperties": [], "typeOfFlow": "Other flow", "classification": {"classHierarchy": "Größen / Umweltliche Größen / EPD EN 15804 / LCI Indikatoren", "name": "GaBiCategories"}}]}, "LCIAResults": {"LCIAResult": [{"referenceToLCIAMethodDataSet": {"shortDescription": [{"value": "Abiotic depletion potential - non-fossil resources (ADPE)", "lang": "en"}, {"value": "Potenzial für die Verknappung abiotischer Ressourcen – nicht fossile Ressourcen (ADPE)", "lang": "de"}], "type": "LCIA method data set", "refObjectId": "b2ad6494-c78d-11e6-9d9d-cec0c932ce01", "version": "01.00.011", "uri": "../lciamethods/b2ad6494-c78d-11e6-9d9d-cec0c932ce01.xml"}, "meanAmount": 0.0, "other": {"anies": [{"value": "1.34E-5", "module": "A1", "scenario": "Standard scenario"}, {"value": "6.15E-7", "module": "A2", "scenario": "Standard scenario"}, {"value": "6.54E-7", "module": "A3", "scenario": "Standard scenario"}, {"value": "5.24E-8", "module": "C1", "scenario": "Standard scenario"}, {"value": "3.41E-7", "module": "C2", "scenario": "Standard scenario"}, {"value": "0.0", "module": "C3", "scenario": "Standard scenario"}, {"value": "4.81E-8", "module": "C4", "scenario": "Standard scenario"}, {"value": "2.69E-7", "module": "D", "scenario": "Standard scenario"}, {"name": "referenceToUnitGroupDataSet", "value": {"shortDescription": [{"value": "kg Sb-eq.", "lang": "en"}], "type": "unit group data set", "refObjectId": "54ccd2d9-a32a-4fc2-923d-f2c8c93e89d4", "version": "30.00.000", "uri": "../unitgroups/54ccd2d9-a32a-4fc2-923d-f2c8c93e89d4.xml"}}]}}, {"referenceToLCIAMethodDataSet": {"shortDescription": [{"value": "Abiotic depletion potential - fossil resources (ADPF)", "lang": "en"}, {"value": "Potenzial für die Verknappung abiotischer Ressourcen – fossile Brennstoffe (ADPF)", "lang": "de"}], "type": "LCIA method data set", "refObjectId": "b2ad6110-c78d-11e6-9d9d-cec0c932ce01", "version": "01.00.011", "uri": "../lciamethods/b2ad6110-c78d-11e6-9d9d-cec0c932ce01.xml"}, "meanAmount": 0.0, "other": {"anies": [{"value": "3.38", "module": "A1", "scenario": "Standard scenario"}, {"value": "0.366", "module": "A2", "scenario": "Standard scenario"}, {"value": "0.956", "module": "A3", "scenario": "Standard scenario"}, {"value": "0.47", "module": "C1", "scenario": "Standard scenario"}, {"value": "0.203", "module": "C2", "scenario": "Standard scenario"}, {"value": "0.0", "module": "C3", "scenario": "Standard scenario"}, {"value": "0.147", "module": "C4", "scenario": "Standard scenario"}, {"value": "0.225", "module": "D", "scenario": "Standard scenario"}, {"name": "referenceToUnitGroupDataSet", "value": {"shortDescription": [{"value": "MJ", "lang": "en"}], "type": "unit group data set", "refObjectId": "93a60a57-a3c8-11da-a746-0800200c9a66", "version": "03.00.000", "uri": "../unitgroups/93a60a57-a3c8-11da-a746-0800200c9a66.xml"}}]}}, {"referenceToLCIAMethodDataSet": {"shortDescription": [{"value": "Acidification potential, Accumulated Exceedance (AP)", "lang": "en"}, {"value": "Versauerungspotenzial, kumulierte Überschreitung (AP)", "lang": "de"}], "type": "LCIA method data set", "refObjectId": "b5c611c6-def3-11e6-bf01-fe55135034f3", "version": "01.03.010", "uri": "../lciamethods/b5c611c6-def3-11e6-bf01-fe55135034f3.xml"}, "meanAmount": 0.0, "other": {"anies": [{"value": "0.00165", "module": "A1", "scenario": "Standard scenario"}, {"value": "1.41E-4", "module": "A2", "scenario": "Standard scenario"}, {"value": "1.8E-4", "module": "A3", "scenario": "Standard scenario"}, {"value": "1.74E-4", "module": "C1", "scenario": "Standard scenario"}, {"value": "7.81E-5", "module": "C2", "scenario": "Standard scenario"}, {"value": "0.0", "module": "C3", "scenario": "Standard scenario"}, {"value": "4.99E-5", "module": "C4", "scenario": "Standard scenario"}, {"value": "6.59E-5", "module": "D", "scenario": "Standard scenario"}, {"name": "referenceToUnitGroupDataSet", "value": {"shortDescription": [{"value": "mol H+-eq.", "lang": "en"}], "type": "unit group data set", "refObjectId": "42e089ac-92bf-4bf2-8ca1-5fc40d18f2ed", "version": "00.01.000", "uri": "../unitgroups/42e089ac-92bf-4bf2-8ca1-5fc40d18f2ed.xml"}}]}}, {"referenceToLCIAMethodDataSet": {"shortDescription": [{"value": "Eutrophication potential - freshwater (EP-freshwater)", "lang": "en"}, {"value": "Eutrophierungspotenzial - Süßwasser (EP-freshwater)", "lang": "de"}], "type": "LCIA method data set", "refObjectId": "b53ec18f-7377-4ad3-86eb-cc3f4f276b2b", "version": "01.00.011", "uri": "../lciamethods/b53ec18f-7377-4ad3-86eb-cc3f4f276b2b.xml"}, "meanAmount": 0.0, "other": {"anies": [{"value": "8.12E-6", "module": "A1", "scenario": "Standard scenario"}, {"value": "2.45E-7", "module": "A2", "scenario": "Standard scenario"}, {"value": "4.71E-6", "module": "A3", "scenario": "Standard scenario"}, {"value": "1.24E-7", "module": "C1", "scenario": "Standard scenario"}, {"value": "1.36E-7", "module": "C2", "scenario": "Standard scenario"}, {"value": "0.0", "module": "C3", "scenario": "Standard scenario"}, {"value": "5.89E-8", "module": "C4", "scenario": "Standard scenario"}, {"value": "3.23E-7", "module": "D", "scenario": "Standard scenario"}, {"name": "referenceToUnitGroupDataSet", "value": {"shortDescription": [{"value": "kg P-eq.", "lang": "en"}], "type": "unit group data set", "refObjectId": "0429039d-a61d-4590-ba67-aa4a20a810a1", "version": "30.00.000", "uri": "../unitgroups/0429039d-a61d-4590-ba67-aa4a20a810a1.xml"}}]}}, {"referenceToLCIAMethodDataSet": {"shortDescription": [{"value": "Eutrophication potential - marine (EP-marine)", "lang": "en"}, {"value": "Eutrophierungspotenzial - Salzwasser (EP-marine)", "lang": "de"}], "type": "LCIA method data set", "refObjectId": "b5c619fa-def3-11e6-bf01-fe55135034f3", "version": "02.00.011", "uri": "../lciamethods/b5c619fa-def3-11e6-bf01-fe55135034f3.xml"}, "meanAmount": 0.0, "other": {"anies": [{"value": "3.04E-4", "module": "A1", "scenario": "Standard scenario"}, {"value": "4.96E-5", "module": "A2", "scenario": "Standard scenario"}, {"value": "3.66E-5", "module": "A3", "scenario": "Standard scenario"}, {"value": "6.69E-5", "module": "C1", "scenario": "Standard scenario"}, {"value": "2.75E-5", "module": "C2", "scenario": "Standard scenario"}, {"value": "0.0", "module": "C3", "scenario": "Standard scenario"}, {"value": "1.72E-5", "module": "C4", "scenario": "Standard scenario"}, {"value": "1.88E-5", "module": "D", "scenario": "Standard scenario"}, {"name": "referenceToUnitGroupDataSet", "value": {"shortDescription": [{"value": "kg N-eq.", "lang": "en"}], "type": "unit group data set", "refObjectId": "d05bb823-ecdf-4686-8c40-bf1d9257859f", "version": "00.00.003", "uri": "../unitgroups/d05bb823-ecdf-4686-8c40-bf1d9257859f.xml"}}]}}, {"referenceToLCIAMethodDataSet": {"shortDescription": [{"value": "Eutrophication potential - terrestrial (EP-terrestrial)", "lang": "en"}, {"value": "Eutrophierungspotenzial - Land (EP-terrestrial)", "lang": "de"}], "type": "LCIA method data set", "refObjectId": "b5c614d2-def3-11e6-bf01-fe55135034f3", "version": "01.02.010", "uri": "../lciamethods/b5c614d2-def3-11e6-bf01-fe55135034f3.xml"}, "meanAmount": 0.0, "other": {"anies": [{"value": "0.00385", "module": "A1", "scenario": "Standard scenario"}, {"value": "5.47E-4", "module": "A2", "scenario": "Standard scenario"}, {"value": "4.92E-4", "module": "A3", "scenario": "Standard scenario"}, {"value": "7.37E-4", "module": "C1", "scenario": "Standard scenario"}, {"value": "3.04E-4", "module": "C2", "scenario": "Standard scenario"}, {"value": "0.0", "module": "C3", "scenario": "Standard scenario"}, {"value": "1.89E-4", "module": "C4", "scenario": "Standard scenario"}, {"value": "2.17E-4", "module": "D", "scenario": "Standard scenario"}, {"name": "referenceToUnitGroupDataSet", "value": {"shortDescription": [{"value": "mol N-eq.", "lang": "en"}], "type": "unit group data set", "refObjectId": "71b4d617-0ec9-4d3f-b65e-e438940c2401", "version": "00.00.003", "uri": "../unitgroups/71b4d617-0ec9-4d3f-b65e-e438940c2401.xml"}}]}}, {"referenceToLCIAMethodDataSet": {"shortDescription": [{"value": "Global Warming Potential - total (GWP-total)", "lang": "en"}, {"value": "Globales Erwärmungspotenzial - total (GWP-total)", "lang": "de"}], "type": "LCIA method data set", "refObjectId": "6a37f984-a4b3-458a-a20a-64418c145fa2", "version": "04.00.017", "uri": "../lciamethods/6a37f984-a4b3-458a-a20a-64418c145fa2.xml"}, "meanAmount": 0.0, "other": {"anies": [{"value": "0.404", "module": "A1", "scenario": "Standard scenario"}, {"value": "0.0243", "module": "A2", "scenario": "Standard scenario"}, {"value": "0.071", "module": "A3", "scenario": "Standard scenario"}, {"value": "0.0345", "module": "C1", "scenario": "Standard scenario"}, {"value": "0.0135", "module": "C2", "scenario": "Standard scenario"}, {"value": "0.0", "module": "C3", "scenario": "Standard scenario"}, {"value": "0.00527", "module": "C4", "scenario": "Standard scenario"}, {"value": "0.0277", "module": "D", "scenario": "Standard scenario"}, {"name": "referenceToUnitGroupDataSet", "value": {"shortDescription": [{"value": "kg CO2-eq.", "lang": "en"}], "type": "unit group data set", "refObjectId": "1ebf3012-d0db-4de2-aefd-ef30cedb0be1", "version": "30.00.000", "uri": "../unitgroups/1ebf3012-d0db-4de2-aefd-ef30cedb0be1.xml"}}]}}, {"referenceToLCIAMethodDataSet": {"shortDescription": [{"value": "Global Warming Potential - fossil fuels (GWP-fossil)", "lang": "en"}, {"value": "Globales Erwärmungspotenzial - fossil (GWP-fossil)", "lang": "de"}], "type": "LCIA method data set", "refObjectId": "5f635281-343e-44fb-83df-1971b155e6b6", "version": "01.00.009", "uri": "../lciamethods/5f635281-343e-44fb-83df-1971b155e6b6.xml"}, "meanAmount": 0.0, "other": {"anies": [{"value": "0.402", "module": "A1", "scenario": "Standard scenario"}, {"value": "0.0243", "module": "A2", "scenario": "Standard scenario"}, {"value": "0.0687", "module": "A3", "scenario": "Standard scenario"}, {"value": "0.0344", "module": "C1", "scenario": "Standard scenario"}, {"value": "0.0135", "module": "C2", "scenario": "Standard scenario"}, {"value": "0.0", "module": "C3", "scenario": "Standard scenario"}, {"value": "0.00526", "module": "C4", "scenario": "Standard scenario"}, {"value": "0.0276", "module": "D", "scenario": "Standard scenario"}, {"name": "referenceToUnitGroupDataSet", "value": {"shortDescription": [{"value": "kg CO2-eq.", "lang": "en"}], "type": "unit group data set", "refObjectId": "1ebf3012-d0db-4de2-aefd-ef30cedb0be1", "version": "30.00.000", "uri": "../unitgroups/1ebf3012-d0db-4de2-aefd-ef30cedb0be1.xml"}}]}}, {"referenceToLCIAMethodDataSet": {"shortDescription": [{"value": "Global Warming Potential - biogenic (GWP-biogenic)", "lang": "en"}, {"value": "Globales Erwärmungspotenzial - biogen (GWP-biogenic)", "lang": "de"}], "type": "LCIA method data set", "refObjectId": "2356e1ab-0185-4db5-86e5-16de51c7485c", "version": "01.00.006", "uri": "../lciamethods/2356e1ab-0185-4db5-86e5-16de51c7485c.xml"}, "meanAmount": 0.0, "other": {"anies": [{"value": "0.00233", "module": "A1", "scenario": "Standard scenario"}, {"value": "1.12E-5", "module": "A2", "scenario": "Standard scenario"}, {"value": "0.00218", "module": "A3", "scenario": "Standard scenario"}, {"value": "9.5E-6", "module": "C1", "scenario": "Standard scenario"}, {"value": "6.22E-6", "module": "C2", "scenario": "Standard scenario"}, {"value": "0.0", "module": "C3", "scenario": "Standard scenario"}, {"value": "1.04E-5", "module": "C4", "scenario": "Standard scenario"}, {"value": "1.29E-4", "module": "D", "scenario": "Standard scenario"}, {"name": "referenceToUnitGroupDataSet", "value": {"shortDescription": [{"value": "kg CO2-eq.", "lang": "en"}], "type": "unit group data set", "refObjectId": "1ebf3012-d0db-4de2-aefd-ef30cedb0be1", "version": "30.00.000", "uri": "../unitgroups/1ebf3012-d0db-4de2-aefd-ef30cedb0be1.xml"}}]}}, {"referenceToLCIAMethodDataSet": {"shortDescription": [{"value": "Global Warming Potential - land use and land use change (GWP-luluc)", "lang": "en"}, {"value": "Globales Erwärmungspotenzial - luluc (GWP-luluc)", "lang": "de"}], "type": "LCIA method data set", "refObjectId": "4331bbdb-978a-490d-8707-eeb047f01a55", "version": "01.00.006", "uri": "../lciamethods/4331bbdb-978a-490d-8707-eeb047f01a55.xml"}, "meanAmount": 0.0, "other": {"anies": [{"value": "1.09E-4", "module": "A1", "scenario": "Standard scenario"}, {"value": "8.9E-6", "module": "A2", "scenario": "Standard scenario"}, {"value": "4.1E-5", "module": "A3", "scenario": "Standard scenario"}, {"value": "2.69E-6", "module": "C1", "scenario": "Standard scenario"}, {"value": "4.94E-6", "module": "C2", "scenario": "Standard scenario"}, {"value": "0.0", "module": "C3", "scenario": "Standard scenario"}, {"value": "1.47E-6", "module": "C4", "scenario": "Standard scenario"}, {"value": "6.53E-6", "module": "D", "scenario": "Standard scenario"}, {"name": "referenceToUnitGroupDataSet", "value": {"shortDescription": [{"value": "kg CO2-eq.", "lang": "en"}], "type": "unit group data set", "refObjectId": "1ebf3012-d0db-4de2-aefd-ef30cedb0be1", "version": "30.00.000", "uri": "../unitgroups/1ebf3012-d0db-4de2-aefd-ef30cedb0be1.xml"}}]}}, {"referenceToLCIAMethodDataSet": {"shortDescription": [{"value": "Depletion potential of the stratospheric ozone layer (ODP)", "lang": "en"}, {"value": "Abbaupotenzial der stratosphärischen Ozonschicht (ODP)", "lang": "de"}], "type": "LCIA method data set", "refObjectId": "b5c629d6-def3-11e6-bf01-fe55135034f3", "version": "02.00.013", "uri": "../lciamethods/b5c629d6-def3-11e6-bf01-fe55135034f3.xml"}, "meanAmount": 0.0, "other": {"anies": [{"value": "2.64E-8", "module": "A1", "scenario": "Standard scenario"}, {"value": "5.36E-9", "module": "A2", "scenario": "Standard scenario"}, {"value": "5.59E-9", "module": "A3", "scenario": "Standard scenario"}, {"value": "7.38E-9", "module": "C1", "scenario": "Standard scenario"}, {"value": "2.97E-9", "module": "C2", "scenario": "Standard scenario"}, {"value": "0.0", "module": "C3", "scenario": "Standard scenario"}, {"value": "2.16E-9", "module": "C4", "scenario": "Standard scenario"}, {"value": "2.0E-9", "module": "D", "scenario": "Standard scenario"}, {"name": "referenceToUnitGroupDataSet", "value": {"shortDescription": [{"value": "kg CFC-11-eq.", "lang": "en"}], "type": "unit group data set", "refObjectId": "d9e957c9-7309-4474-bf3a-7777df6c4e5b", "version": "25.00.000", "uri": "../unitgroups/d9e957c9-7309-4474-bf3a-7777df6c4e5b.xml"}}]}}, {"referenceToLCIAMethodDataSet": {"shortDescription": [{"value": "Photochemical Ozone Creation Potential (POCP)", "lang": "en"}, {"value": "Bildungspotenzial für troposphärisches Ozon (POCP)", "lang": "de"}], "type": "LCIA method data set", "refObjectId": "b5c610fe-def3-11e6-bf01-fe55135034f3", "version": "02.00.015", "uri": "../lciamethods/b5c610fe-def3-11e6-bf01-fe55135034f3.xml"}, "meanAmount": 0.0, "other": {"anies": [{"value": "0.00108", "module": "A1", "scenario": "Standard scenario"}, {"value": "1.56E-4", "module": "A2", "scenario": "Standard scenario"}, {"value": "1.18E-4", "module": "A3", "scenario": "Standard scenario"}, {"value": "2.08E-4", "module": "C1", "scenario": "Standard scenario"}, {"value": "8.67E-5", "module": "C2", "scenario": "Standard scenario"}, {"value": "0.0", "module": "C3", "scenario": "Standard scenario"}, {"value": "5.5E-5", "module": "C4", "scenario": "Standard scenario"}, {"value": "6.15E-5", "module": "D", "scenario": "Standard scenario"}, {"name": "referenceToUnitGroupDataSet", "value": {"shortDescription": [{"value": "kg NMVOC-eq.", "lang": "en"}], "type": "unit group data set", "refObjectId": "d27c25f8-fbc1-44c6-b47b-4adbae4199c6", "version": "00.00.003", "uri": "../unitgroups/d27c25f8-fbc1-44c6-b47b-4adbae4199c6.xml"}}]}}, {"referenceToLCIAMethodDataSet": {"shortDescription": [{"value": "Water (user) deprivation potential (WDP)", "lang": "en"}, {"value": "Wasser-Entzugspotenzial (Benutzer) (WDP)", "lang": "de"}], "type": "LCIA method data set", "refObjectId": "b2ad66ce-c78d-11e6-9d9d-cec0c932ce01", "version": "03.00.015", "uri": "../lciamethods/b2ad66ce-c78d-11e6-9d9d-cec0c932ce01.xml"}, "meanAmount": 0.0, "other": {"anies": [{"value": "0.0466", "module": "A1", "scenario": "Standard scenario"}, {"value": "0.00131", "module": "A2", "scenario": "Standard scenario"}, {"value": "0.00938", "module": "A3", "scenario": "Standard scenario"}, {"value": "6.3E-4", "module": "C1", "scenario": "Standard scenario"}, {"value": "7.27E-4", "module": "C2", "scenario": "Standard scenario"}, {"value": "0.0", "module": "C3", "scenario": "Standard scenario"}, {"value": "0.00659", "module": "C4", "scenario": "Standard scenario"}, {"value": "0.00107", "module": "D", "scenario": "Standard scenario"}, {"name": "referenceToUnitGroupDataSet", "value": {"shortDescription": [{"value": "m3 world eq. deprived", "lang": "en"}], "type": "unit group data set", "refObjectId": "6ae2df01-888e-46c8-b17d-49fa3869b476", "version": "00.00.003", "uri": "../unitgroups/6ae2df01-888e-46c8-b17d-49fa3869b476.xml"}}]}}, {"referenceToLCIAMethodDataSet": {"shortDescription": [{"value": "Potential incidence of disease due to PM emissions (PM)", "lang": "en"}, {"value": "Potenzielles Auftreten von Krankheiten aufgrund von Feinstaubemissionen (PM)", "lang": "de"}], "type": "LCIA method data set", "refObjectId": "b5c602c6-def3-11e6-bf01-fe55135034f3", "version": "02.00.012", "uri": "../lciamethods/b5c602c6-def3-11e6-bf01-fe55135034f3.xml"}, "meanAmount": 0.0, "other": {"anies": [{"value": "5.94E-8", "module": "A1", "scenario": "Standard scenario"}, {"value": "2.19E-9", "module": "A2", "scenario": "Standard scenario"}, {"value": "2.51E-9", "module": "A3", "scenario": "Standard scenario"}, {"value": "2.72E-9", "module": "C1", "scenario": "Standard scenario"}, {"value": "1.21E-9", "module": "C2", "scenario": "Standard scenario"}, {"value": "0.0", "module": "C3", "scenario": "Standard scenario"}, {"value": "9.7E-10", "module": "C4", "scenario": "Standard scenario"}, {"value": "1.72E-9", "module": "D", "scenario": "Standard scenario"}, {"name": "referenceToUnitGroupDataSet", "value": {"shortDescription": [{"value": "Disease incidence", "lang": "en"}], "type": "unit group data set", "refObjectId": "3883559b-648f-4afc-8ba2-0bd24f3affa3", "version": "00.00.003", "uri": "../unitgroups/3883559b-648f-4afc-8ba2-0bd24f3affa3.xml"}}]}}, {"referenceToLCIAMethodDataSet": {"shortDescription": [{"value": "Potential Human exposure efficiency relative to U235 (IRP)", "lang": "en"}, {"value": "Potenzielle Wirkung durch Exposition des Menschen mit U235 (IRP)", "lang": "de"}], "type": "LCIA method data set", "refObjectId": "b5c632be-def3-11e6-bf01-fe55135034f3", "version": "01.00.012", "uri": "../lciamethods/b5c632be-def3-11e6-bf01-fe55135034f3.xml"}, "meanAmount": 0.0, "other": {"anies": [{"value": "0.00797", "module": "A1", "scenario": "Standard scenario"}, {"value": "0.00153", "module": "A2", "scenario": "Standard scenario"}, {"value": "0.00233", "module": "A3", "scenario": "Standard scenario"}, {"value": "0.00201", "module": "C1", "scenario": "Standard scenario"}, {"value": "8.51E-4", "module": "C2", "scenario": "Standard scenario"}, {"value": "0.0", "module": "C3", "scenario": "Standard scenario"}, {"value": "6.03E-4", "module": "C4", "scenario": "Standard scenario"}, {"value": "3.75E-4", "module": "D", "scenario": "Standard scenario"}, {"name": "referenceToUnitGroupDataSet", "value": {"shortDescription": [{"value": "kgBq U235-eq.", "lang": "en"}], "type": "unit group data set", "refObjectId": "456b05bf-1415-44a9-9993-02452f554c09", "version": "00.00.003", "uri": "../unitgroups/456b05bf-1415-44a9-9993-02452f554c09.xml"}}]}}, {"referenceToLCIAMethodDataSet": {"shortDescription": [{"value": "Potential Comparative Toxic Unit for ecosystems (ETP-fw)", "lang": "en"}, {"value": "Potenzielle Toxizitätsvergleichseinheit für Ökosysteme (ETP-fw)", "lang": "de"}], "type": "LCIA method data set", "refObjectId": "ee1082d1-b0f7-43ca-a1f0-21e2a4a74511", "version": "01.00.003", "uri": "../lciamethods/ee1082d1-b0f7-43ca-a1f0-21e2a4a74511.xml"}, "meanAmount": 0.0, "other": {"anies": [{"value": "8.67", "module": "A1", "scenario": "Standard scenario"}, {"value": "0.327", "module": "A2", "scenario": "Standard scenario"}, {"value": "0.809", "module": "A3", "scenario": "Standard scenario"}, {"value": "0.283", "module": "C1", "scenario": "Standard scenario"}, {"value": "0.181", "module": "C2", "scenario": "Standard scenario"}, {"value": "0.0", "module": "C3", "scenario": "Standard scenario"}, {"value": "0.0953", "module": "C4", "scenario": "Standard scenario"}, {"value": "0.679", "module": "D", "scenario": "Standard scenario"}, {"name": "referenceToUnitGroupDataSet", "value": {"shortDescription": [{"value": "CTUe", "lang": "en"}], "type": "unit group data set", "refObjectId": "aa959ded-f1eb-4efb-9c5c-2d60be36b3e6", "version": "00.00.003", "uri": "../unitgroups/aa959ded-f1eb-4efb-9c5c-2d60be36b3e6.xml"}}]}}, {"referenceToLCIAMethodDataSet": {"shortDescription": [{"value": "Potential Comparative Toxic Unit for humans - cancer effects (HTP-c)", "lang": "en"}, {"value": "Potenzielle Toxizitätsvergleichseinheit für den Menschen - kanzerogene Wirkung (HTP-c)", "lang": "de"}], "type": "LCIA method data set", "refObjectId": "2299222a-bbd8-474f-9d4f-4dd1f18aea7c", "version": "01.00.004", "uri": "../lciamethods/2299222a-bbd8-474f-9d4f-4dd1f18aea7c.xml"}, "meanAmount": 0.0, "other": {"anies": [{"value": "6.69E-10", "module": "A1", "scenario": "Standard scenario"}, {"value": "1.06E-11", "module": "A2", "scenario": "Standard scenario"}, {"value": "3.21E-11", "module": "A3", "scenario": "Standard scenario"}, {"value": "3.02E-11", "module": "C1", "scenario": "Standard scenario"}, {"value": "5.88E-12", "module": "C2", "scenario": "Standard scenario"}, {"value": "0.0", "module": "C3", "scenario": "Standard scenario"}, {"value": "2.2E-12", "module": "C4", "scenario": "Standard scenario"}, {"value": "5.13E-11", "module": "D", "scenario": "Standard scenario"}, {"name": "referenceToUnitGroupDataSet", "value": {"shortDescription": [{"value": "CTUh", "lang": "en"}], "type": "unit group data set", "refObjectId": "d4c9523e-2d7e-49fd-8469-998f547d3a70", "version": "00.00.003", "uri": "../unitgroups/d4c9523e-2d7e-49fd-8469-998f547d3a70.xml"}}]}}, {"referenceToLCIAMethodDataSet": {"shortDescription": [{"value": "Potential Comparative Toxic Unit for humans - non-cancer effects (HTP-nc)", "lang": "en"}, {"value": "Potenzielle Toxizitätsvergleichseinheit für den Menschen - nicht kanzerogene Wirkung (HTP-nc)", "lang": "de"}], "type": "LCIA method data set", "refObjectId": "3af763a5-b7a1-48c9-9cee-1f223481fcef", "version": "01.00.003", "uri": "../lciamethods/3af763a5-b7a1-48c9-9cee-1f223481fcef.xml"}, "meanAmount": 0.0, "other": {"anies": [{"value": "9.97E-9", "module": "A1", "scenario": "Standard scenario"}, {"value": "3.57E-10", "module": "A2", "scenario": "Standard scenario"}, {"value": "7.0E-10", "module": "A3", "scenario": "Standard scenario"}, {"value": "2.33E-10", "module": "C1", "scenario": "Standard scenario"}, {"value": "1.98E-10", "module": "C2", "scenario": "Standard scenario"}, {"value": "0.0", "module": "C3", "scenario": "Standard scenario"}, {"value": "6.77E-11", "module": "C4", "scenario": "Standard scenario"}, {"value": "9.43E-10", "module": "D", "scenario": "Standard scenario"}, {"name": "referenceToUnitGroupDataSet", "value": {"shortDescription": [{"value": "CTUh", "lang": "en"}], "type": "unit group data set", "refObjectId": "d4c9523e-2d7e-49fd-8469-998f547d3a70", "version": "00.00.003", "uri": "../unitgroups/d4c9523e-2d7e-49fd-8469-998f547d3a70.xml"}}]}}, {"referenceToLCIAMethodDataSet": {"shortDescription": [{"value": "Potential Soil quality index (SQP)", "lang": "en"}, {"value": "Potenzieller Bodenqualitätsindex (SQP)", "lang": "de"}], "type": "LCIA method data set", "refObjectId": "b2ad6890-c78d-11e6-9d9d-cec0c932ce01", "version": "01.00.011", "uri": "../lciamethods/b2ad6890-c78d-11e6-9d9d-cec0c932ce01.xml"}, "meanAmount": 0.0, "other": {"anies": [{"value": "1.66", "module": "A1", "scenario": "Standard scenario"}, {"value": "0.318", "module": "A2", "scenario": "Standard scenario"}, {"value": "0.629", "module": "A3", "scenario": "Standard scenario"}, {"value": "0.06", "module": "C1", "scenario": "Standard scenario"}, {"value": "0.176", "module": "C2", "scenario": "Standard scenario"}, {"value": "0.0", "module": "C3", "scenario": "Standard scenario"}, {"value": "0.308", "module": "C4", "scenario": "Standard scenario"}, {"value": "0.031", "module": "D", "scenario": "Standard scenario"}, {"name": "referenceToUnitGroupDataSet", "value": {"shortDescription": [{"value": "dimensionless", "lang": "en"}], "type": "unit group data set", "refObjectId": "f130951c-e67f-4f7f-8dd4-665de3974e18", "version": "00.00.004", "uri": "../unitgroups/f130951c-e67f-4f7f-8dd4-665de3974e18.xml"}}]}}]}, "otherAttributes": {"{http://www.indata.network/EPD/2019}epd-version": "1.2", "{http://www.okworx.com/ILCD/Extensions/2018/Profile}profile": "EN_15804_A2"}, "version": "1.1"}