{"processInformation": {"dataSetInformation": {"UUID": "c836b484-773f-4a07-9baa-c70da743ccea", "name": {"baseName": [{"value": "Glued laminated timber - special shapes (German average)", "lang": "en"}, {"value": "Brettschichtholz - Sonderformen (Durchschnitt DE)", "lang": "de"}], "functionalUnitFlowProperties": [{"lang": "de"}]}, "synonyms": [{"lang": "de"}], "classificationInformation": {"classification": [{"class": [{"value": "Holz", "level": 0, "classId": "3"}, {"value": "Vollholz", "level": 1, "classId": "3.1"}, {"value": "Brettschichtholz (BSH)", "level": 2, "classId": "3.1.04"}], "name": "OEKOBAU.DAT"}]}, "generalComment": [{"value": "Weitere Informationen zur deklarierten Einheit (Zusammensetzung) und die auf Herstellerangaben beruhende Sachbilanz (In- und Output der Stoff- und Energieströme) stehen als Excel-Datei unter dem Unterpunkt Hintergrund-Bericht zum Download bereit.\r\nDer Datensatz wurde 2023 als Aktualisierung mit gleichbleibendem Vordergrundsystem erstellt. Alle Hintergrunddaten entstammen der GaBi Professional Datenbank in der Content Version 2023.1. Die Modellierung und Berechnung der Ökobilanz basiert auf den europäischen Normen EN 15804:2012+A2:2019 und EN 16485:2014. Bei Rückfragen wenden Sie sich bitte an holzundklima@thuenen.de.", "lang": "de"}, {"value": "Further information on the declared unit and the inventory analysis based on manufacturer information (input and output of material and energy flows) are available for download as an Excel file within the section “background info”.\r\nThe data set was created in 2021 as an update with identical foreground system. All background data sets are taken from the GaBi Professional Database with content version 2021.1. The modeling and calculation of the life cycle assessment is based on the European standards EN 15804:2012+A2:2019 and EN 16485:2014. For questions, please contact holzundklima@thuenen.de.", "lang": "en"}], "referenceToExternalDocumentation": [{"shortDescription": [{"value": "Rüter S, Diederichs S (2012) Ökobilanz Basisdaten für Bauprodukte aus Holz, Hamburg, Johann Heinrich von Thünen Institut, Institut für Holztechnologie und Holzbiologie, Abschlussbericht", "lang": "en"}], "type": "source data set", "refObjectId": "caead862-97ea-4e99-9b3c-438c78c79ebd", "version": "00.00.004", "uri": "http://openlca.org/ilcd/resource/sources/caead862-97ea-4e99-9b3c-438c78c79ebd"}, {"shortDescription": [{"value": "LCI_BSH_sond_xlsx", "lang": "en"}], "type": "source data set", "refObjectId": "fe335984-f13d-48b9-a952-30cd2514c55b", "version": "01.01.001", "uri": "http://openlca.org/ilcd/resource/sources/fe335984-f13d-48b9-a952-30cd2514c55b"}], "other": {"anies": ["<olca:modules xmlns:olca=\"http://openlca.org/epd_ilcd\" xmlns=\"http://lca.jrc.it/ILCD/Process\" xmlns:c=\"http://lca.jrc.it/ILCD/Contact\" xmlns:common=\"http://lca.jrc.it/ILCD/Common\" xmlns:epd2=\"http://www.indata.network/EPD/2019\" xmlns:f=\"http://lca.jrc.it/ILCD/Flow\" xmlns:fp=\"http://lca.jrc.it/ILCD/FlowProperty\" xmlns:m=\"http://lca.jrc.it/ILCD/LCIAMethod\" xmlns:ns9=\"http://www.okworx.com/ILCD/Extensions/2018/Profile\" xmlns:s=\"http://lca.jrc.it/ILCD/Source\" xmlns:u=\"http://lca.jrc.it/ILCD/UnitGroup\"><olca:module olca:name=\"A1\"/><olca:module olca:name=\"A2\"/><olca:module olca:name=\"A3\"/><olca:module olca:name=\"A1-A3\"/><olca:module olca:name=\"A5\" olca:scenario=\"Entsorgung Verpackung\">Das Modul A5 enthält ausschließlich die Entsorgung der Verpackungsmaterialien</olca:module><olca:module olca:name=\"C2\"/><olca:module olca:name=\"C3\"/><olca:module olca:name=\"D\" olca:scenario=\"energetisch\">therm. Verwertung</olca:module><olca:module olca:name=\"D\" olca:scenario=\"stofflich\">stoffl. Verwertung</olca:module>\n                </olca:modules>", "<olca:modules xmlns:olca=\"http://openlca.org/epd_ilcd\" xmlns=\"http://lca.jrc.it/ILCD/Process\" xmlns:c=\"http://lca.jrc.it/ILCD/Contact\" xmlns:common=\"http://lca.jrc.it/ILCD/Common\" xmlns:epd2=\"http://www.indata.network/EPD/2019\" xmlns:f=\"http://lca.jrc.it/ILCD/Flow\" xmlns:fp=\"http://lca.jrc.it/ILCD/FlowProperty\" xmlns:m=\"http://lca.jrc.it/ILCD/LCIAMethod\" xmlns:ns9=\"http://www.okworx.com/ILCD/Extensions/2018/Profile\" xmlns:s=\"http://lca.jrc.it/ILCD/Source\" xmlns:u=\"http://lca.jrc.it/ILCD/UnitGroup\"><olca:module olca:name=\"A1\"/><olca:module olca:name=\"A2\"/><olca:module olca:name=\"A3\"/><olca:module olca:name=\"A1-A3\"/><olca:module olca:name=\"A5\" olca:scenario=\"Entsorgung Verpackung\">Das Modul A5 enthält ausschließlich die Entsorgung der Verpackungsmaterialien</olca:module><olca:module olca:name=\"C2\"/><olca:module olca:name=\"C3\"/><olca:module olca:name=\"D\" olca:scenario=\"energetisch\">therm. Verwertung</olca:module><olca:module olca:name=\"D\" olca:scenario=\"stofflich\">stoffl. Verwertung</olca:module>\n                </olca:modules>", "<olca:modules xmlns:olca=\"http://openlca.org/epd_ilcd\" xmlns=\"http://lca.jrc.it/ILCD/Process\" xmlns:c=\"http://lca.jrc.it/ILCD/Contact\" xmlns:common=\"http://lca.jrc.it/ILCD/Common\" xmlns:epd2=\"http://www.indata.network/EPD/2019\" xmlns:f=\"http://lca.jrc.it/ILCD/Flow\" xmlns:fp=\"http://lca.jrc.it/ILCD/FlowProperty\" xmlns:m=\"http://lca.jrc.it/ILCD/LCIAMethod\" xmlns:ns9=\"http://www.okworx.com/ILCD/Extensions/2018/Profile\" xmlns:s=\"http://lca.jrc.it/ILCD/Source\" xmlns:u=\"http://lca.jrc.it/ILCD/UnitGroup\"><olca:module olca:name=\"A1\"/><olca:module olca:name=\"A2\"/><olca:module olca:name=\"A3\"/><olca:module olca:name=\"A1-A3\"/><olca:module olca:name=\"A5\" olca:scenario=\"Entsorgung Verpackung\">Das Modul A5 enthält ausschließlich die Entsorgung der Verpackungsmaterialien</olca:module><olca:module olca:name=\"C2\"/><olca:module olca:name=\"C3\"/><olca:module olca:name=\"D\" olca:scenario=\"energetisch\">therm. Verwertung</olca:module><olca:module olca:name=\"D\" olca:scenario=\"stofflich\">stoffl. Verwertung</olca:module>\n                </olca:modules>", "<olca:modules xmlns:olca=\"http://openlca.org/epd_ilcd\" xmlns=\"http://lca.jrc.it/ILCD/Process\" xmlns:c=\"http://lca.jrc.it/ILCD/Contact\" xmlns:common=\"http://lca.jrc.it/ILCD/Common\" xmlns:epd2=\"http://www.indata.network/EPD/2019\" xmlns:f=\"http://lca.jrc.it/ILCD/Flow\" xmlns:fp=\"http://lca.jrc.it/ILCD/FlowProperty\" xmlns:m=\"http://lca.jrc.it/ILCD/LCIAMethod\" xmlns:ns9=\"http://www.okworx.com/ILCD/Extensions/2018/Profile\" xmlns:s=\"http://lca.jrc.it/ILCD/Source\" xmlns:u=\"http://lca.jrc.it/ILCD/UnitGroup\"><olca:module olca:name=\"A1\"/><olca:module olca:name=\"A2\"/><olca:module olca:name=\"A3\"/><olca:module olca:name=\"A1-A3\"/><olca:module olca:name=\"A5\" olca:scenario=\"Entsorgung Verpackung\">Das Modul A5 enthält ausschließlich die Entsorgung der Verpackungsmaterialien</olca:module><olca:module olca:name=\"C2\"/><olca:module olca:name=\"C3\"/><olca:module olca:name=\"D\" olca:scenario=\"energetisch\">therm. Verwertung</olca:module><olca:module olca:name=\"D\" olca:scenario=\"stofflich\">stoffl. Verwertung</olca:module>\n                </olca:modules>", {"scenario": [{"description": [{"value": "therm. Verwertung"}], "name": "energetisch", "group": "Modul D", "default": true}, {"description": [{"value": "stoffl. Verwertung"}], "name": "stofflich", "group": "Modul D"}, {"description": [{"value": "Das Modul A5 enthält ausschließlich die Entsorgung der Verpackungsmaterialien"}], "name": "Entsorgung Verpackung", "group": "Modul A5", "default": true}]}]}}, "quantitativeReference": {"referenceToReferenceFlow": [0], "type": "Reference flow(s)"}, "time": {"referenceYear": 2023, "dataSetValidUntil": 2028, "timeRepresentativenessDescription": [{"value": "Der Datensatz basiert auf Produktionsdaten aus den Jahren 2009 bis 2011 (Vordergrundsystem).\r\nEine Aktualisierung des Hintergrundsystems erfolgte 2023.", "lang": "de"}, {"value": "The data set is based on production data from the years 2009 to 2011 (foreground system).\r\nThe background system was updated in 2021.", "lang": "en"}]}, "geography": {"locationOfOperationSupplyOrProduction": {"descriptionOfRestrictions": [{"value": "Für die Ökobilanzierung von Brettschichtholz, Sonderformen wurden Daten von 7 Werken berücksichtigt (Rüter & Diederichs 2012).  Für alle in Rüter & Diederichs (2012) angeführten Vollholzprodukte wurden von 2009 bis 2011 insgesamt 178 Prozesslinien erfasst. Im Verhältnis zu den vom Statistischen Bundesamt gemeldeten Produktionsmengen im selben Zeitraum entspricht die erreichte Abdeckung von Vollholzprodukten aus Nadelschnittholz 38 %. ", "lang": "de"}], "location": "DE"}}, "technology": {"technologyDescriptionAndIncludedProcesses": [{"value": "Brettschichtholz besteht aus mindestens drei faserparallel miteinander verklebten getrockneten Brettern oder Brettlamellen (keilgezinktes Konstruktionsvollholz) aus Nadelholz. Die im Folgenden aufgeführten Ergebnisse und Parameter beziehen sich auf gekrümmte horizontal laminierte Träger (Sonderformen). Die Verklebung von Brettschichtholz Sonderformen wird vornehmlich mittels Melamin-Harnstoff-Formaldehyd Bindemitteln durchgeführt. Teilweise werden auch 1 Komponenten Polyurethan-Bindemittel genutzt. Die keilgezinkten Lamellen werden analog zu den Konstruktionsvollhölzern verklebt. Für die Herstellung von Brettschichtholz Sonderformen wird konventionelles Schnittholz zunächst auf etwa 12 % Holzfeuchte getrocknet, vorgehobelt und visuell bzw. maschinell nach Festigkeit sortiert. Identifizierte Brettabschnitte mit festigkeitsvermindernden Stellen werden abhängig von der erwünschten Festigkeitsklasse ausgekappt und die entstandenen Bretter durch Keilzinkenverbindung zu endlos langen Lamellen gestoßen. Im darauffolgenden Vorhobelprozess werden die Lamellen auf bis zu 45 mm Stärke gehobelt, um nach Beleimung der Breitseite im gekrümmten Pressbett zu mindesten 3-lagigen Holzrohlingen verpresst zu werden. Nach Aushärtung wird der Rohling gehobelt, gefast, abgebunden und verpackt.\r\nDie Holzfeuchte des Produktes liegt bei 12%.", "lang": "de"}], "technologicalApplicability": [{"value": "Brettschichtholz wird vorwiegend bei hoher statischer Beanspruchung im Ingenieurholzbau verwendet.", "lang": "de"}, {"value": "Glued laminated timber is mainly used for high structural demands in timber engineering.", "lang": "en"}], "referenceToTechnologyFlowDiagrammOrPicture": [{"shortDescription": [{"value": "Brettschicht_sonder", "lang": "en"}], "type": "source data set", "refObjectId": "9982e38b-4cd3-4cdd-aeee-8f6c9f092494", "version": "00.00.001", "uri": "http://openlca.org/ilcd/resource/sources/9982e38b-4cd3-4cdd-aeee-8f6c9f092494"}]}}, "modellingAndValidation": {"LCIMethodAndAllocation": {"typeOfDataSet": "EPD", "referenceToLCAMethodDetails": [{"shortDescription": [{"value": "EN 15804", "lang": "de"}, {"value": "EN 15804", "lang": "en"}], "type": "source data set", "refObjectId": "b00f9ec0-7874-11e3-981f-0800200c9a66", "version": "00.02.001"}, {"shortDescription": [{"value": "ILCD format", "lang": "en"}], "type": "source data set", "refObjectId": "a97a0155-0234-4b87-b4ce-a45da52f2a40", "version": "03.00.000", "uri": "http://lca.jrc.ec.europa.eu/lcainfohub/datasets/ilcd/sources/a97a0155-0234-4b87-b4ce-a45da52f2a40.xml"}], "other": {"anies": [{"name": "subType", "value": "representative dataset"}]}}, "dataSourcesTreatmentAndRepresentativeness": {"referenceToDataSource": [{"shortDescription": [{"value": "Rüter S, Diederichs S (2012) Ökobilanz Basisdaten für Bauprodukte aus Holz, Hamburg, Johann Heinrich von Thünen Institut, Institut für Holztechnologie und Holzbiologie, Abschlussbericht", "lang": "en"}], "type": "source data set", "refObjectId": "caead862-97ea-4e99-9b3c-438c78c79ebd", "version": "00.00.004", "uri": "http://openlca.org/ilcd/resource/sources/caead862-97ea-4e99-9b3c-438c78c79ebd"}, {"shortDescription": [{"value": "GaBi database (general)", "lang": "en"}], "type": "source data set", "refObjectId": "28d74cc0-db8b-4d7e-bc44-5f6d56ce0c4a", "version": "00.03.002"}], "useAdviceForDataSet": [{"value": "Aufgrund der hohen Abdeckung bildet der Datensatz die durchschnittlichen Produktionsverhältnisse und die damit verbundenen Umweltwirkungen repräsentativ für Deutschland ab. Liegen keine herstellerspezifischen Ökobilanzergebnisse des verwendeten Produkts vor, empfiehlt sich die Verwendung dieses Durchschnittsdatensatzes.", "lang": "de"}]}, "validation": {"review": [{"referenceToNameOfReviewerAndInstitution": [{"shortDescription": [{"value": "Dr. Frank Werner - Umwelt & Entwicklung", "lang": "de"}], "type": "contact data set", "refObjectId": "62792478-795c-4ae2-ac9a-1012d9515424", "version": "00.02.000"}], "otherReviewDetails": [{"lang": "de"}], "type": "Independent external review"}]}, "complianceDeclarations": {"compliance": [{"referenceToComplianceSystem": {"shortDescription": [{"value": "EN 15804+A2", "lang": "de"}, {"value": "EN 15804+A2", "lang": "en"}], "type": "source data set", "refObjectId": "c0016b33-8cf7-415c-ac6e-deba0d21440d", "version": "00.01.000"}}, {"referenceToComplianceSystem": {"shortDescription": [{"value": "EN 16485", "lang": "de"}], "type": "source data set", "refObjectId": "56c9c859-d469-424f-80ac-ac909332dd21", "version": "00.00.001"}}]}}, "administrativeInformation": {"dataGenerator": {"referenceToPersonOrEntityGeneratingTheDataSet": [{"shortDescription": [{"value": "Thünen-Institut für Holzforschung", "lang": "en"}], "type": "contact data set", "refObjectId": "7ac81002-181b-4302-827e-7ccc1a3730f0", "version": "00.01.000"}]}, "dataEntryBy": {"timeStamp": 1685111605021, "referenceToDataSetFormat": [{"shortDescription": [{"value": "ILCD format", "lang": "en"}], "type": "source data set", "refObjectId": "a97a0155-0234-4b87-b4ce-a45da52f2a40", "version": "03.00.000", "uri": "http://lca.jrc.ec.europa.eu/lcainfohub/datasets/ilcd/sources/a97a0155-0234-4b87-b4ce-a45da52f2a40.xml"}, {"shortDescription": [{"value": "EPD Data Format Extensions v1.2", "lang": "en"}, {"value": "EPD-Datenformaterweiterungen v1.2", "lang": "de"}], "type": "source data set", "refObjectId": "a29449fd-aa2f-4de8-b5d7-4b06b43c6fde", "version": "00.01.000"}], "referenceToPersonOrEntityEnteringTheData": {"shortDescription": [{"value": "Thünen-Institut für Holzforschung", "lang": "en"}], "type": "contact data set", "refObjectId": "7ac81002-181b-4302-827e-7ccc1a3730f0", "version": "00.01.000"}}, "publicationAndOwnership": {"dataSetVersion": "00.00.030", "referenceToPrecedingDataSetVersion": [{"shortDescription": [{"value": "Brettschichtholz - Sonderformen (Durchschnitt DE 2022_A2)", "lang": "de"}, {"value": "Glued laminated timber - special shapes (German average)", "lang": "en"}], "type": "process data set", "refObjectId": "da69ac98-1dfa-4fd3-89ce-219c4cc6f385", "version": "00.00.028"}], "referenceToRegistrationAuthority": {"shortDescription": [{"value": "Thünen-Institut für Holzforschung", "lang": "en"}], "type": "contact data set", "refObjectId": "7ac81002-181b-4302-827e-7ccc1a3730f0", "version": "00.01.000"}, "referenceToOwnershipOfDataSet": {"shortDescription": [{"value": "Thünen-Institut für Holzforschung", "lang": "en"}], "type": "contact data set", "refObjectId": "7ac81002-181b-4302-827e-7ccc1a3730f0", "version": "00.01.000"}, "copyright": true, "licenseType": "Free of charge for all users and uses", "accessRestrictions": [{"lang": "de"}], "other": {"anies": [{"name": "referenceToPublisher", "value": {"shortDescription": [{"value": "The Federal Institute for Research on Building, Urban Affairs and Spatial Development (BBSR) within the Federal Office for Building and Regional Planning (BBR)", "lang": "en"}, {"value": "Bundesinstitut für Bau-, Stadt- und Raumforschung (BBSR) im Bundesamt für Bauwesen und Raumordnung (BBR)", "lang": "de"}], "type": "contact data set", "refObjectId": "f11651e0-7877-11e3-981f-0800200c9a66", "version": "00.01.000"}}]}}}, "exchanges": {"exchange": [{"dataSetInternalID": 0, "referenceToFlowDataSet": {"shortDescription": [{"value": "Brettschichtholz (Sonderform)", "lang": "de"}], "type": "flow data set", "refObjectId": "995eb782-6e79-49c4-84bb-8e0821c366e9", "version": "00.00.005", "uri": "http://openlca.org/ilcd/resource/flows/995eb782-6e79-49c4-84bb-8e0821c366e9"}, "meanAmount": 1.0, "resultingAmount": 1.0, "referenceFlow": true, "resultingflowAmount": 1.0, "flowProperties": [{"name": [{"lang": "en", "value": "Carbon content (biogenic) - packaging"}], "uuid": "262a541b-209e-44cc-a426-33bce30de7b1", "meanValue": 0.0}, {"name": [{"lang": "en", "value": "Carbon content (biogenic)"}], "uuid": "62e503ce-544a-4599-b2ad-bcea15a7bf20", "meanValue": 221.3}, {"name": [{"lang": "en", "value": "Volume"}, {"lang": "de", "value": "Volumen"}], "uuid": "93a60a56-a3c8-22da-a746-0800200c9a66", "referenceFlowProperty": true, "meanValue": 1.0, "referenceUnit": "m3", "unitGroupUUID": "cd950537-0a98-4044-9ba7-9f9a68d0a504"}, {"name": [{"lang": "en", "value": "Mass"}, {"lang": "de", "value": "Masse"}], "uuid": "93a60a56-a3c8-11da-a746-0800200b9a66", "meanValue": 508.43}], "materialProperties": [{"name": "gross density", "value": "508.43", "unit": "kg/m^3", "unitDescription": "kilograms per cubic metre"}], "typeOfFlow": "Product flow", "classification": {"classHierarchy": "Holz / Vollholz / Brettschichtholz", "name": "ilcd"}}, {"dataSetInternalID": 1, "referenceToFlowDataSet": {"shortDescription": [{"value": "Use of renewable primary energy (PERE)", "lang": "en"}, {"value": "Erneuerbare Primärenergie als Energieträger (PERE)", "lang": "de"}, {"value": "Uso de energía primaria renovable excluyendo los recursos de energía primaria renovable utilizada como materia prima (PERE)", "lang": "es"}], "type": "flow data set", "refObjectId": "20f32be5-0398-4288-9b6d-accddd195317", "version": "30.00.000"}, "exchange direction": "INPUT", "meanAmount": 0.0, "other": {"anies": [{"value": "930.8253788632826", "module": "A1"}, {"value": "25.73828200622388", "module": "A2"}, {"value": "1801.5467347156193", "module": "A3"}, {"value": "2758.110395585126", "module": "A1-A3"}, {"value": "0.080239921184098", "module": "A5", "scenario": "Entsorgung Verpackung"}, {"value": "0.658010113584976", "module": "C2"}, {"value": "131.426809221954", "module": "C3"}, {"value": "5315.337488524768", "module": "D", "scenario": "energetisch"}, {"value": "-37.707109251464935", "module": "D", "scenario": "stofflich"}, {"name": "referenceToUnitGroupDataSet", "value": {"shortDescription": [{"value": "MJ"}], "type": "unit group data set", "refObjectId": "93a60a57-a3c8-11da-a746-0800200c9a66", "uri": "../unitgroups/93a60a57-a3c8-11da-a746-0800200c9a66"}}]}, "flowProperties": [], "typeOfFlow": "Other flow", "classification": {"classHierarchy": "Größen / Umweltliche Größen / EPD EN 15804 / LCI Indikatoren", "name": "GaBiCategories"}}, {"dataSetInternalID": 2, "referenceToFlowDataSet": {"shortDescription": [{"value": "Use of renewable primary energy resources used as raw materials (PERM)", "lang": "en"}, {"value": "Erneuerbare Primärenergie zur stofflichen Nutzung (PERM)", "lang": "de"}, {"value": "Uso de energía primaria renovable utilizada como materia prima (PERM)", "lang": "es"}], "type": "flow data set", "refObjectId": "fb3ec0de-548d-4508-aea5-00b73bf6f702", "version": "30.00.000"}, "exchange direction": "INPUT", "meanAmount": 0.0, "other": {"anies": [{"value": "8529.15189", "module": "A1"}, {"value": "0.0", "module": "A2"}, {"value": "0.0", "module": "A3"}, {"value": "8529.15189", "module": "A1-A3"}, {"value": "0.0", "module": "A5", "scenario": "Entsorgung Verpackung"}, {"value": "0.0", "module": "C2"}, {"value": "-8529.15189", "module": "C3"}, {"value": "0.0", "module": "D", "scenario": "energetisch"}, {"value": "0.0", "module": "D", "scenario": "stofflich"}, {"name": "referenceToUnitGroupDataSet", "value": {"shortDescription": [{"value": "MJ"}], "type": "unit group data set", "refObjectId": "93a60a57-a3c8-11da-a746-0800200c9a66", "uri": "../unitgroups/93a60a57-a3c8-11da-a746-0800200c9a66"}}]}, "flowProperties": [], "typeOfFlow": "Other flow", "classification": {"classHierarchy": "Größen / Umweltliche Größen / EPD EN 15804 / LCI Indikatoren", "name": "GaBiCategories"}}, {"dataSetInternalID": 3, "referenceToFlowDataSet": {"shortDescription": [{"value": "Total use of renewable primary energy resources (PERT)", "lang": "en"}, {"value": "Total erneuerbare Primärenergie (PERT)", "lang": "de"}, {"value": "Uso total de la energía primaria renovable (energía primaria y recursos de energía primaria renovable utilizada como materia prima) (PERT)", "lang": "es"}], "type": "flow data set", "refObjectId": "53f97275-fa8a-4cdd-9024-65936002acd0", "version": "30.00.000"}, "exchange direction": "INPUT", "meanAmount": 0.0, "other": {"anies": [{"value": "9459.977268863282", "module": "A1"}, {"value": "25.73828200622388", "module": "A2"}, {"value": "1801.5467347156193", "module": "A3"}, {"value": "11287.262285585124", "module": "A1-A3"}, {"value": "0.080239921184098", "module": "A5", "scenario": "Entsorgung Verpackung"}, {"value": "0.658010113584976", "module": "C2"}, {"value": "-8397.725080778046", "module": "C3"}, {"value": "5315.337488524768", "module": "D", "scenario": "energetisch"}, {"value": "-37.707109251464935", "module": "D", "scenario": "stofflich"}, {"name": "referenceToUnitGroupDataSet", "value": {"shortDescription": [{"value": "MJ"}], "type": "unit group data set", "refObjectId": "93a60a57-a3c8-11da-a746-0800200c9a66", "uri": "../unitgroups/93a60a57-a3c8-11da-a746-0800200c9a66"}}]}, "flowProperties": [], "typeOfFlow": "Other flow", "classification": {"classHierarchy": "Größen / Umweltliche Größen / EPD EN 15804 / LCI Indikatoren", "name": "GaBiCategories"}}, {"dataSetInternalID": 4, "referenceToFlowDataSet": {"shortDescription": [{"value": "Use of non renewable primary energy (PENRE)", "lang": "en"}, {"value": "Nicht-erneuerbare Primärenergie als Energieträger (PENRE)", "lang": "de"}, {"value": "Uso de energía primaria no renovable, excluyendo los recursos de energía primaria no renovable utilizada como materia prima (PENRE)", "lang": "es"}], "type": "flow data set", "refObjectId": "ac857178-2b45-46ec-892a-a9a4332f0372", "version": "30.00.000"}, "exchange direction": "INPUT", "meanAmount": 0.0, "other": {"anies": [{"value": "781.4884906294651", "module": "A1"}, {"value": "368.7210955129943", "module": "A2"}, {"value": "929.4099330739976", "module": "A3"}, {"value": "2079.619519216457", "module": "A1-A3"}, {"value": "21.51202627993037", "module": "A5", "scenario": "Entsorgung Verpackung"}, {"value": "9.32135918495101", "module": "C2"}, {"value": "139.715142765093", "module": "C3"}, {"value": "-4087.5034324367", "module": "D", "scenario": "energetisch"}, {"value": "-152.06161691293948", "module": "D", "scenario": "stofflich"}, {"name": "referenceToUnitGroupDataSet", "value": {"shortDescription": [{"value": "MJ"}], "type": "unit group data set", "refObjectId": "93a60a57-a3c8-11da-a746-0800200c9a66", "uri": "../unitgroups/93a60a57-a3c8-11da-a746-0800200c9a66"}}]}, "flowProperties": [], "typeOfFlow": "Other flow", "classification": {"classHierarchy": "Größen / Umweltliche Größen / EPD EN 15804 / LCI Indikatoren", "name": "GaBiCategories"}}, {"dataSetInternalID": 5, "referenceToFlowDataSet": {"shortDescription": [{"value": "Use of non renewable primary energy resources used as raw materials (PENRM)", "lang": "en"}, {"value": "Nicht-erneuerbare Primärenergie zur stofflichen Nutzung (PENRM)", "lang": "de"}, {"value": "Uso de la energía primaria no renovable utilizada como materia prima (PENRM)", "lang": "es"}], "type": "flow data set", "refObjectId": "1421caa0-679d-4bf4-b282-0eb850ccae27", "version": "30.00.000"}, "exchange direction": "INPUT", "meanAmount": 0.0, "other": {"anies": [{"value": "127.2795213529878", "module": "A1"}, {"value": "0.0", "module": "A2"}, {"value": "21.204", "module": "A3"}, {"value": "148.4835213529878", "module": "A1-A3"}, {"value": "-21.204", "module": "A5", "scenario": "Entsorgung Verpackung"}, {"value": "0.0", "module": "C2"}, {"value": "-127.27952135298779", "module": "C3"}, {"value": "0.0", "module": "D", "scenario": "energetisch"}, {"value": "0.0", "module": "D", "scenario": "stofflich"}, {"name": "referenceToUnitGroupDataSet", "value": {"shortDescription": [{"value": "MJ"}], "type": "unit group data set", "refObjectId": "93a60a57-a3c8-11da-a746-0800200c9a66", "uri": "../unitgroups/93a60a57-a3c8-11da-a746-0800200c9a66"}}]}, "flowProperties": [], "typeOfFlow": "Other flow", "classification": {"classHierarchy": "Größen / Umweltliche Größen / EPD EN 15804 / LCI Indikatoren", "name": "GaBiCategories"}}, {"dataSetInternalID": 6, "referenceToFlowDataSet": {"shortDescription": [{"value": "Total use of non renewable primary energy resource (PENRT)", "lang": "en"}, {"value": "Total nicht erneuerbare Primärenergie (PENRT)", "lang": "de"}, {"value": "Uso total de la energía primaria no renovable (energía primaria y recursos de energía primaria renovable utilizada como materia prima) (PENRT)", "lang": "es"}], "type": "flow data set", "refObjectId": "06159210-646b-4c8d-8583-da9b3b95a6c1", "version": "30.00.000"}, "exchange direction": "INPUT", "meanAmount": 0.0, "other": {"anies": [{"value": "908.7680119824529", "module": "A1"}, {"value": "368.7210955129943", "module": "A2"}, {"value": "950.6139330739976", "module": "A3"}, {"value": "2228.1030405694446", "module": "A1-A3"}, {"value": "0.30802627993037035", "module": "A5", "scenario": "Entsorgung Verpackung"}, {"value": "9.32135918495101", "module": "C2"}, {"value": "12.435621412105206", "module": "C3"}, {"value": "-4087.5034324367", "module": "D", "scenario": "energetisch"}, {"value": "-152.06161691293948", "module": "D", "scenario": "stofflich"}, {"name": "referenceToUnitGroupDataSet", "value": {"shortDescription": [{"value": "MJ"}], "type": "unit group data set", "refObjectId": "93a60a57-a3c8-11da-a746-0800200c9a66", "uri": "../unitgroups/93a60a57-a3c8-11da-a746-0800200c9a66"}}]}, "flowProperties": [], "typeOfFlow": "Other flow", "classification": {"classHierarchy": "Größen / Umweltliche Größen / EPD EN 15804 / LCI Indikatoren", "name": "GaBiCategories"}}, {"dataSetInternalID": 7, "referenceToFlowDataSet": {"shortDescription": [{"value": "Use of secondary material (SM)", "lang": "en"}, {"value": "Einsatz von Sekundärstoffen (SM)", "lang": "de"}, {"value": "Uso de materiales secundarios (SM)", "lang": "es"}], "type": "flow data set", "refObjectId": "c6a1f35f-2d09-4f54-8dfb-97e502e1ce92", "version": "30.00.000"}, "exchange direction": "INPUT", "meanAmount": 0.0, "other": {"anies": [{"value": "0.0", "module": "A1"}, {"value": "0.0", "module": "A2"}, {"value": "0.0", "module": "A3"}, {"value": "0.0", "module": "A1-A3"}, {"value": "0.0", "module": "A5", "scenario": "Entsorgung Verpackung"}, {"value": "0.0", "module": "C2"}, {"value": "0.0", "module": "C3"}, {"value": "0.0", "module": "D", "scenario": "energetisch"}, {"value": "508.5078759607983", "module": "D", "scenario": "stofflich"}, {"name": "referenceToUnitGroupDataSet", "value": {"shortDescription": [{"value": "kg"}], "type": "unit group data set", "refObjectId": "ad38d542-3fe9-439d-9b95-2f5f7752acaf", "uri": "../unitgroups/ad38d542-3fe9-439d-9b95-2f5f7752acaf"}}]}, "flowProperties": [], "typeOfFlow": "Other flow", "classification": {"classHierarchy": "Größen / Umweltliche Größen / EPD EN 15804 / LCI Indikatoren", "name": "GaBiCategories"}}, {"dataSetInternalID": 8, "referenceToFlowDataSet": {"shortDescription": [{"value": "Use of renewable secondary fuels (RSF)", "lang": "en"}, {"value": "Erneuerbare Sekundärbrennstoffe (RSF)", "lang": "de"}, {"value": "Uso de combustibles secundarios renovables (RSF)", "lang": "es"}], "type": "flow data set", "refObjectId": "64333088-a55f-4aa2-9a31-c10b07816787", "version": "30.00.000"}, "exchange direction": "INPUT", "meanAmount": 0.0, "other": {"anies": [{"value": "56.915071707460136", "module": "A1"}, {"value": "0.0", "module": "A2"}, {"value": "84.51233069996543", "module": "A3"}, {"value": "141.42740240742557", "module": "A1-A3"}, {"value": "0.0", "module": "A5", "scenario": "Entsorgung Verpackung"}, {"value": "0.0", "module": "C2"}, {"value": "0.0", "module": "C3"}, {"value": "0.0", "module": "D", "scenario": "energetisch"}, {"value": "0.0", "module": "D", "scenario": "stofflich"}, {"name": "referenceToUnitGroupDataSet", "value": {"shortDescription": [{"value": "MJ"}], "type": "unit group data set", "refObjectId": "93a60a57-a3c8-11da-a746-0800200c9a66", "uri": "../unitgroups/93a60a57-a3c8-11da-a746-0800200c9a66"}}]}, "flowProperties": [], "typeOfFlow": "Other flow", "classification": {"classHierarchy": "Größen / Umweltliche Größen / EPD EN 15804 / LCI Indikatoren", "name": "GaBiCategories"}}, {"dataSetInternalID": 9, "referenceToFlowDataSet": {"shortDescription": [{"value": "Use of non renewable secondary fuels (NRSF)", "lang": "en"}, {"value": "Nicht erneuerbare Sekundärbrennstoffe (NRSF)", "lang": "de"}, {"value": "Uso de combustibles secundarios no renovables (NRSF)", "lang": "es"}], "type": "flow data set", "refObjectId": "89def144-d39a-4287-b86f-efde453ddcb2", "version": "30.00.000"}, "exchange direction": "INPUT", "meanAmount": 0.0, "other": {"anies": [{"value": "0.0", "module": "A1"}, {"value": "0.0", "module": "A2"}, {"value": "0.0", "module": "A3"}, {"value": "0.0", "module": "A1-A3"}, {"value": "0.0", "module": "A5", "scenario": "Entsorgung Verpackung"}, {"value": "0.0", "module": "C2"}, {"value": "0.0", "module": "C3"}, {"value": "0.0", "module": "D", "scenario": "energetisch"}, {"value": "0.0", "module": "D", "scenario": "stofflich"}, {"name": "referenceToUnitGroupDataSet", "value": {"shortDescription": [{"value": "MJ"}], "type": "unit group data set", "refObjectId": "93a60a57-a3c8-11da-a746-0800200c9a66", "uri": "../unitgroups/93a60a57-a3c8-11da-a746-0800200c9a66"}}]}, "flowProperties": [], "typeOfFlow": "Other flow", "classification": {"classHierarchy": "Größen / Umweltliche Größen / EPD EN 15804 / LCI Indikatoren", "name": "GaBiCategories"}}, {"dataSetInternalID": 10, "referenceToFlowDataSet": {"shortDescription": [{"value": "Use of net fresh water (FW)", "lang": "en"}, {"value": "Einsatz von Süßwasserressourcen (FW)", "lang": "de"}, {"value": "Uso neto de recursos de agua dulce (FW)", "lang": "es"}], "type": "flow data set", "refObjectId": "3cf952c8-f3a4-461d-8c96-96456ca62246", "version": "30.00.000"}, "exchange direction": "INPUT", "meanAmount": 0.0, "other": {"anies": [{"value": "0.1485406507823704", "module": "A1"}, {"value": "0.02740264524214419", "module": "A2"}, {"value": "0.25711676363635", "module": "A3"}, {"value": "0.4330600596608646", "module": "A1-A3"}, {"value": "0.00397374631663949", "module": "A5", "scenario": "Entsorgung Verpackung"}, {"value": "7.25105792993116E-4", "module": "C2"}, {"value": "0.0460593600990649", "module": "C3"}, {"value": "0.926665205404396", "module": "D", "scenario": "energetisch"}, {"value": "-0.01735918861460875", "module": "D", "scenario": "stofflich"}, {"name": "referenceToUnitGroupDataSet", "value": {"shortDescription": [{"value": "m3"}], "type": "unit group data set", "refObjectId": "cd950537-0a98-4044-9ba7-9f9a68d0a504", "uri": "../unitgroups/cd950537-0a98-4044-9ba7-9f9a68d0a504"}}]}, "flowProperties": [], "typeOfFlow": "Other flow", "classification": {"classHierarchy": "Größen / Umweltliche Größen / EPD EN 15804 / LCI Indikatoren", "name": "GaBiCategories"}}, {"dataSetInternalID": 11, "referenceToFlowDataSet": {"shortDescription": [{"value": "Hazardous waste disposed (HWD)", "lang": "en"}, {"value": "Gefährlicher Abfall zur Deponie (HWD)", "lang": "de"}, {"value": "Residuos peligrosos eliminados (HWD)", "lang": "es"}], "type": "flow data set", "refObjectId": "430f9e0f-59b2-46a0-8e0d-55e0e84948fc", "version": "30.00.000"}, "exchange direction": "OUTPUT", "meanAmount": 0.0, "other": {"anies": [{"value": "2.7520335306093006E-7", "module": "A1"}, {"value": "1.2658732461255707E-9", "module": "A2"}, {"value": "9.80868442185179E-7", "module": "A3"}, {"value": "1.2573376684922346E-6", "module": "A1-A3"}, {"value": "4.29753154869589E-12", "module": "A5", "scenario": "Entsorgung Verpackung"}, {"value": "3.4490122266594E-11", "module": "C2"}, {"value": "-2.73017504570204E-8", "module": "C3"}, {"value": "4.360793851499538E-7", "module": "D", "scenario": "energetisch"}, {"value": "4.86904422376094E-9", "module": "D", "scenario": "stofflich"}, {"name": "referenceToUnitGroupDataSet", "value": {"shortDescription": [{"value": "kg"}], "type": "unit group data set", "refObjectId": "ad38d542-3fe9-439d-9b95-2f5f7752acaf", "uri": "../unitgroups/ad38d542-3fe9-439d-9b95-2f5f7752acaf"}}]}, "flowProperties": [], "typeOfFlow": "Other flow", "classification": {"classHierarchy": "Größen / Umweltliche Größen / EPD EN 15804 / LCI Indikatoren", "name": "GaBiCategories"}}, {"dataSetInternalID": 12, "referenceToFlowDataSet": {"shortDescription": [{"value": "Non hazardous waste dispose (NHWD)", "lang": "en"}, {"value": "Entsorgter nicht gefährlicher Abfall (NHWD)", "lang": "de"}, {"value": "Residuos no peligrosos eliminados (NHWD)", "lang": "es"}], "type": "flow data set", "refObjectId": "b29ef66b-e286-4afa-949f-62f1a7b4d7fa", "version": "30.00.000"}, "exchange direction": "OUTPUT", "meanAmount": 0.0, "other": {"anies": [{"value": "0.8939785391225192", "module": "A1"}, {"value": "0.05343256136987228", "module": "A2"}, {"value": "1.5072034784114987", "module": "A3"}, {"value": "2.4546145789038905", "module": "A1-A3"}, {"value": "0.00977791874694415", "module": "A5", "scenario": "Entsorgung Verpackung"}, {"value": "0.0013434429701811", "module": "C2"}, {"value": "0.128150630908692", "module": "C3"}, {"value": "9.16756992175053", "module": "D", "scenario": "energetisch"}, {"value": "-0.0405419883900337", "module": "D", "scenario": "stofflich"}, {"name": "referenceToUnitGroupDataSet", "value": {"shortDescription": [{"value": "kg"}], "type": "unit group data set", "refObjectId": "ad38d542-3fe9-439d-9b95-2f5f7752acaf", "uri": "../unitgroups/ad38d542-3fe9-439d-9b95-2f5f7752acaf"}}]}, "flowProperties": [], "typeOfFlow": "Other flow", "classification": {"classHierarchy": "Größen / Umweltliche Größen / EPD EN 15804 / LCI Indikatoren", "name": "GaBiCategories"}}, {"dataSetInternalID": 13, "referenceToFlowDataSet": {"shortDescription": [{"value": "Radioactive waste disposed (RWD)", "lang": "en"}, {"value": "Entsorgter radioaktiver Abfall (RWD)", "lang": "de"}, {"value": "Residuos radiactivos eliminados (RWD)", "lang": "es"}], "type": "flow data set", "refObjectId": "3449546e-52ad-4b39-b809-9fb77cea8ff6", "version": "30.00.000"}, "exchange direction": "OUTPUT", "meanAmount": 0.0, "other": {"anies": [{"value": "0.019838600731417466", "module": "A1"}, {"value": "5.031307367580358E-4", "module": "A2"}, {"value": "0.07182717029871269", "module": "A3"}, {"value": "0.09216890176688819", "module": "A1-A3"}, {"value": "8.13159596319503E-6", "module": "A5", "scenario": "Entsorgung Verpackung"}, {"value": "1.2052023290931E-5", "module": "C2"}, {"value": "0.0136289435846902", "module": "C3"}, {"value": "-0.3174619624824434", "module": "D", "scenario": "energetisch"}, {"value": "-0.0032878868344714926", "module": "D", "scenario": "stofflich"}, {"name": "referenceToUnitGroupDataSet", "value": {"shortDescription": [{"value": "kg"}], "type": "unit group data set", "refObjectId": "ad38d542-3fe9-439d-9b95-2f5f7752acaf", "uri": "../unitgroups/ad38d542-3fe9-439d-9b95-2f5f7752acaf"}}]}, "flowProperties": [], "typeOfFlow": "Other flow", "classification": {"classHierarchy": "Größen / Umweltliche Größen / EPD EN 15804 / LCI Indikatoren", "name": "GaBiCategories"}}, {"dataSetInternalID": 14, "referenceToFlowDataSet": {"shortDescription": [{"value": "Components for re-use (CRU)", "lang": "en"}, {"value": "Komponenten für die Wiederverwendung (CRU)", "lang": "de"}, {"value": "Componentes para su reutilización (CRU)", "lang": "es"}], "type": "flow data set", "refObjectId": "a2b32f97-3fc7-4af2-b209-525bc6426f33", "version": "30.00.000"}, "exchange direction": "OUTPUT", "meanAmount": 0.0, "other": {"anies": [{"value": "0.0", "module": "A1"}, {"value": "0.0", "module": "A2"}, {"value": "0.0", "module": "A3"}, {"value": "0.0", "module": "A1-A3"}, {"value": "0.0", "module": "A5", "scenario": "Entsorgung Verpackung"}, {"value": "0.0", "module": "C2"}, {"value": "0.0", "module": "C3"}, {"value": "0.0", "module": "D", "scenario": "energetisch"}, {"value": "0.0", "module": "D", "scenario": "stofflich"}, {"name": "referenceToUnitGroupDataSet", "value": {"shortDescription": [{"value": "kg"}], "type": "unit group data set", "refObjectId": "ad38d542-3fe9-439d-9b95-2f5f7752acaf", "uri": "../unitgroups/ad38d542-3fe9-439d-9b95-2f5f7752acaf"}}]}, "flowProperties": [], "typeOfFlow": "Other flow", "classification": {"classHierarchy": "Größen / Umweltliche Größen / EPD EN 15804 / LCI Indikatoren", "name": "GaBiCategories"}}, {"dataSetInternalID": 15, "referenceToFlowDataSet": {"shortDescription": [{"value": "Materials for recycling (MFR)", "lang": "en"}, {"value": "Stoffe zum Recycling (MFR)", "lang": "de"}, {"value": "Materiales para el reciclaje (MFR)", "lang": "es"}], "type": "flow data set", "refObjectId": "d7fe48a5-4103-49c8-9aae-b0b5dfdbd6ae", "version": "30.00.000"}, "exchange direction": "OUTPUT", "meanAmount": 0.0, "other": {"anies": [{"value": "0.0", "module": "A1"}, {"value": "0.0", "module": "A2"}, {"value": "0.0", "module": "A3"}, {"value": "0.0", "module": "A1-A3"}, {"value": "0.0", "module": "A5", "scenario": "Entsorgung Verpackung"}, {"value": "0.0", "module": "C2"}, {"value": "508.5078759607983", "module": "C3"}, {"value": "0.0", "module": "D", "scenario": "energetisch"}, {"value": "0.0", "module": "D", "scenario": "stofflich"}, {"name": "referenceToUnitGroupDataSet", "value": {"shortDescription": [{"value": "kg"}], "type": "unit group data set", "refObjectId": "ad38d542-3fe9-439d-9b95-2f5f7752acaf", "uri": "../unitgroups/ad38d542-3fe9-439d-9b95-2f5f7752acaf"}}]}, "flowProperties": [], "typeOfFlow": "Other flow", "classification": {"classHierarchy": "Größen / Umweltliche Größen / EPD EN 15804 / LCI Indikatoren", "name": "GaBiCategories"}}, {"dataSetInternalID": 16, "referenceToFlowDataSet": {"shortDescription": [{"value": "Materials for energy recovery (MER)", "lang": "en"}, {"value": "Stoffe für die Energierückgewinnung (MER)", "lang": "de"}, {"value": "Materiales para valorización energética (recuperación de energía) (MER)", "lang": "es"}], "type": "flow data set", "refObjectId": "59a9181c-3aaf-46ee-8b13-2b3723b6e447", "version": "30.00.000"}, "exchange direction": "OUTPUT", "meanAmount": 0.0, "other": {"anies": [{"value": "0.0", "module": "A1"}, {"value": "0.0", "module": "A2"}, {"value": "0.0", "module": "A3"}, {"value": "0.0", "module": "A1-A3"}, {"value": "0.0", "module": "A5", "scenario": "Entsorgung Verpackung"}, {"value": "0.0", "module": "C2"}, {"value": "508.5078759607983", "module": "C3"}, {"value": "0.0", "module": "D", "scenario": "energetisch"}, {"value": "0.0", "module": "D", "scenario": "stofflich"}, {"name": "referenceToUnitGroupDataSet", "value": {"shortDescription": [{"value": "kg"}], "type": "unit group data set", "refObjectId": "ad38d542-3fe9-439d-9b95-2f5f7752acaf", "uri": "../unitgroups/ad38d542-3fe9-439d-9b95-2f5f7752acaf"}}]}, "flowProperties": [], "typeOfFlow": "Other flow", "classification": {"classHierarchy": "Größen / Umweltliche Größen / EPD EN 15804 / LCI Indikatoren", "name": "GaBiCategories"}}, {"dataSetInternalID": 17, "referenceToFlowDataSet": {"shortDescription": [{"value": "Exported electrical energy (EEE)", "lang": "en"}, {"value": "Exportierte elektrische Energie (EEE)", "lang": "de"}, {"value": "Energía exportada electrica (EEE)", "lang": "es"}], "type": "flow data set", "refObjectId": "4da0c987-2b76-40d6-9e9e-82a017aaaf29", "version": "30.00.000"}, "exchange direction": "OUTPUT", "meanAmount": 0.0, "other": {"anies": [{"value": "0.0", "module": "A1"}, {"value": "0.0", "module": "A2"}, {"value": "0.158267320312986", "module": "A3"}, {"value": "0.158267320312986", "module": "A1-A3"}, {"value": "3.35828456969107", "module": "A5", "scenario": "Entsorgung Verpackung"}, {"value": "0.0", "module": "C2"}, {"value": "0.0", "module": "C3"}, {"value": "0.0", "module": "D", "scenario": "energetisch"}, {"value": "0.0", "module": "D", "scenario": "stofflich"}, {"name": "referenceToUnitGroupDataSet", "value": {"shortDescription": [{"value": "MJ"}], "type": "unit group data set", "refObjectId": "93a60a57-a3c8-11da-a746-0800200c9a66", "uri": "../unitgroups/93a60a57-a3c8-11da-a746-0800200c9a66"}}]}, "flowProperties": [], "typeOfFlow": "Other flow", "classification": {"classHierarchy": "Größen / Umweltliche Größen / EPD EN 15804 / LCI Indikatoren", "name": "GaBiCategories"}}, {"dataSetInternalID": 18, "referenceToFlowDataSet": {"shortDescription": [{"value": "Exported thermal energy (EET)", "lang": "en"}, {"value": "Exportierte thermische Energie (EET)", "lang": "de"}, {"value": "Energía exportada termal (EET)", "lang": "es"}], "type": "flow data set", "refObjectId": "98daf38a-7a79-46d3-9a37-2b7bd0955810", "version": "30.00.000"}, "exchange direction": "OUTPUT", "meanAmount": 0.0, "other": {"anies": [{"value": "0.0", "module": "A1"}, {"value": "0.0", "module": "A2"}, {"value": "0.367673858494946", "module": "A3"}, {"value": "0.367673858494946", "module": "A1-A3"}, {"value": "7.7346240410552", "module": "A5", "scenario": "Entsorgung Verpackung"}, {"value": "0.0", "module": "C2"}, {"value": "0.0", "module": "C3"}, {"value": "0.0", "module": "D", "scenario": "energetisch"}, {"value": "0.0", "module": "D", "scenario": "stofflich"}, {"name": "referenceToUnitGroupDataSet", "value": {"shortDescription": [{"value": "MJ"}], "type": "unit group data set", "refObjectId": "93a60a57-a3c8-11da-a746-0800200c9a66", "uri": "../unitgroups/93a60a57-a3c8-11da-a746-0800200c9a66"}}]}, "flowProperties": [], "typeOfFlow": "Other flow", "classification": {"classHierarchy": "Größen / Umweltliche Größen / EPD EN 15804 / LCI Indikatoren", "name": "GaBiCategories"}}]}, "LCIAResults": {"LCIAResult": [{"referenceToLCIAMethodDataSet": {"shortDescription": [{"value": "Global Warming Potential - total (GWP-total)", "lang": "en"}, {"value": "Globales Erwärmungspotenzial - total (GWP-total)", "lang": "de"}], "type": "LCIA method data set", "refObjectId": "6a37f984-a4b3-458a-a20a-64418c145fa2", "version": "04.00.017"}, "meanAmount": 0.0, "other": {"anies": [{"value": "-757.2492581369519", "module": "A1"}, {"value": "26.908908213278202", "module": "A2"}, {"value": "67.01400612526376", "module": "A3"}, {"value": "-663.32634379841", "module": "A1-A3"}, {"value": "1.84875629433369", "module": "A5", "scenario": "Entsorgung Verpackung"}, {"value": "0.667413027867962", "module": "C2"}, {"value": "821.3738066041344", "module": "C3"}, {"value": "-219.48026618766252", "module": "D", "scenario": "energetisch"}, {"value": "-11.444364126825741", "module": "D", "scenario": "stofflich"}, {"name": "referenceToUnitGroupDataSet", "value": {"shortDescription": [{"value": "kg CO2-Äqv."}], "type": "unit group data set", "refObjectId": "1ebf3012-d0db-4de2-aefd-ef30cedb0be1", "uri": "../unitgroups/1ebf3012-d0db-4de2-aefd-ef30cedb0be1"}}]}}, {"referenceToLCIAMethodDataSet": {"shortDescription": [{"value": "Global Warming Potential - fossil fuels (GWP-fossil)", "lang": "en"}, {"value": "Globales Erwärmungspotenzial - fossil (GWP-fossil)", "lang": "de"}], "type": "LCIA method data set", "refObjectId": "5f635281-343e-44fb-83df-1971b155e6b6", "version": "01.00.009"}, "meanAmount": 0.0, "other": {"anies": [{"value": "54.16574186304804", "module": "A1"}, {"value": "26.908908213278202", "module": "A2"}, {"value": "67.01400612526376", "module": "A3"}, {"value": "148.08865620159", "module": "A1-A3"}, {"value": "1.84875629433369", "module": "A5", "scenario": "Entsorgung Verpackung"}, {"value": "0.667413027867962", "module": "C2"}, {"value": "9.95880660413445", "module": "C3"}, {"value": "-219.48026618766252", "module": "D", "scenario": "energetisch"}, {"value": "-11.444364126825741", "module": "D", "scenario": "stofflich"}, {"name": "referenceToUnitGroupDataSet", "value": {"shortDescription": [{"value": "kg CO2-Äqv."}], "type": "unit group data set", "refObjectId": "1ebf3012-d0db-4de2-aefd-ef30cedb0be1", "uri": "../unitgroups/1ebf3012-d0db-4de2-aefd-ef30cedb0be1"}}]}}, {"referenceToLCIAMethodDataSet": {"shortDescription": [{"value": "Global Warming Potential - biogenic (GWP-biogenic)", "lang": "en"}, {"value": "Globales Erwärmungspotenzial - biogen (GWP-biogenic)", "lang": "de"}], "type": "LCIA method data set", "refObjectId": "2356e1ab-0185-4db5-86e5-16de51c7485c", "version": "01.00.006"}, "meanAmount": 0.0, "other": {"anies": [{"value": "-811.415", "module": "A1"}, {"value": "0.0", "module": "A2"}, {"value": "0.0", "module": "A3"}, {"value": "-811.415", "module": "A1-A3"}, {"value": "0.0", "module": "A5", "scenario": "Entsorgung Verpackung"}, {"value": "0.0", "module": "C2"}, {"value": "811.415", "module": "C3"}, {"value": "0.0", "module": "D", "scenario": "energetisch"}, {"value": "0.0", "module": "D", "scenario": "stofflich"}, {"name": "referenceToUnitGroupDataSet", "value": {"shortDescription": [{"value": "kg CO2-Äqv."}], "type": "unit group data set", "refObjectId": "1ebf3012-d0db-4de2-aefd-ef30cedb0be1", "uri": "../unitgroups/1ebf3012-d0db-4de2-aefd-ef30cedb0be1"}}]}}, {"referenceToLCIAMethodDataSet": {"shortDescription": [{"value": "Depletion potential of the stratospheric ozone layer (ODP)", "lang": "en"}, {"value": "Abbaupotenzial der stratosphärischen Ozonschicht (ODP)", "lang": "de"}], "type": "LCIA method data set", "refObjectId": "b5c629d6-def3-11e6-bf01-fe55135034f3", "version": "02.00.013", "uri": "http://lca.jrc.ec.europa.eu/lcainfohub/datasets/elcd/lciamethods/8b723200-3d8f-4eec-9e10-444edb029476.xml"}, "meanAmount": 0.0, "other": {"anies": [{"value": "3.355477694744418E-10", "module": "A1"}, {"value": "3.091209294364507E-12", "module": "A2"}, {"value": "1.4014145558644235E-9", "module": "A3"}, {"value": "1.74005353463323E-9", "module": "A1-A3"}, {"value": "1.60049070285756E-13", "module": "A5", "scenario": "Entsorgung Verpackung"}, {"value": "5.98627058663835E-14", "module": "C2"}, {"value": "2.71144025222497E-10", "module": "C3"}, {"value": "-6.439925428971773E-9", "module": "D", "scenario": "energetisch"}, {"value": "-6.450097698205894E-11", "module": "D", "scenario": "stofflich"}, {"name": "referenceToUnitGroupDataSet", "value": {"shortDescription": [{"value": "kg CFC 11-Äquiv."}], "type": "unit group data set", "refObjectId": "d9e957c9-7309-4474-bf3a-7777df6c4e5b", "uri": "../unitgroups/d9e957c9-7309-4474-bf3a-7777df6c4e5b"}}]}}, {"referenceToLCIAMethodDataSet": {"shortDescription": [{"value": "Acidification potential, Accumulated Exceedance (AP)", "lang": "en"}, {"value": "Versauerungspotenzial, kumulierte Überschreitung (AP)", "lang": "de"}], "type": "LCIA method data set", "refObjectId": "b5c611c6-def3-11e6-bf01-fe55135034f3", "version": "01.03.010", "uri": "http://lca.jrc.ec.europa.eu/lcainfohub/datasets/elcd/lciamethods/f6cbd466-253f-4145-a4bb-8dae7d266e89.xml"}, "meanAmount": 0.0, "other": {"anies": [{"value": "0.33117262504806483", "module": "A1"}, {"value": "0.16555457111239458", "module": "A2"}, {"value": "0.3520011675458219", "module": "A3"}, {"value": "0.8487283637062812", "module": "A1-A3"}, {"value": "2.9555186895554E-4", "module": "A5", "scenario": "Entsorgung Verpackung"}, {"value": "0.00419706246552155", "module": "C2"}, {"value": "0.0151465127048372", "module": "C3"}, {"value": "-0.24649399064292662", "module": "D", "scenario": "energetisch"}, {"value": "-0.0690202511595961", "module": "D", "scenario": "stofflich"}, {"name": "referenceToUnitGroupDataSet", "value": {"shortDescription": [{"value": "mol H+ eqv."}], "type": "unit group data set", "refObjectId": "42e089ac-92bf-4bf2-8ca1-5fc40d18f2ed", "uri": "../unitgroups/42e089ac-92bf-4bf2-8ca1-5fc40d18f2ed"}}]}}, {"referenceToLCIAMethodDataSet": {"shortDescription": [{"value": "Eutrophication potential - freshwater (EP-freshwater)", "lang": "en"}, {"value": "Eutrophierungspotenzial - Süßwasser (EP-freshwater)", "lang": "de"}], "type": "LCIA method data set", "refObjectId": "b53ec18f-7377-4ad3-86eb-cc3f4f276b2b", "version": "01.00.011", "uri": "http://lca.jrc.ec.europa.eu/lcainfohub/datasets/elcd/lciamethods/a4630d5b-df2f-48ae-b3f2-5e5257606d68.xml"}, "meanAmount": 0.0, "other": {"anies": [{"value": "1.6278390465479688E-4", "module": "A1"}, {"value": "9.154155267968363E-5", "module": "A2"}, {"value": "3.44256104613418E-4", "module": "A3"}, {"value": "5.985815619478985E-4", "module": "A1-A3"}, {"value": "4.67708745922693E-8", "module": "A5", "scenario": "Entsorgung Verpackung"}, {"value": "2.49311811038568E-6", "module": "C2"}, {"value": "5.92937547569769E-5", "module": "C3"}, {"value": "-0.0013831234906821405", "module": "D", "scenario": "energetisch"}, {"value": "-3.2966119756087096E-5", "module": "D", "scenario": "stofflich"}, {"name": "referenceToUnitGroupDataSet", "value": {"shortDescription": [{"value": "kg P eqv."}], "type": "unit group data set", "refObjectId": "0429039d-a61d-4590-ba67-aa4a20a810a1", "uri": "../unitgroups/0429039d-a61d-4590-ba67-aa4a20a810a1"}}]}}, {"referenceToLCIAMethodDataSet": {"shortDescription": [{"value": "Eutrophication potential - marine (EP-marine)", "lang": "en"}, {"value": "Eutrophierungspotenzial - Salzwasser (EP-marine)", "lang": "de"}], "type": "LCIA method data set", "refObjectId": "b5c619fa-def3-11e6-bf01-fe55135034f3", "version": "02.00.011", "uri": "http://lca.jrc.ec.europa.eu/lcainfohub/datasets/elcd/lciamethods/5296e2be-060b-4e50-b033-d45f85f6ac92.xml"}, "meanAmount": 0.0, "other": {"anies": [{"value": "0.16657132540584924", "module": "A1"}, {"value": "0.08130542934986343", "module": "A2"}, {"value": "0.14712955794652", "module": "A3"}, {"value": "0.39500631270223263", "module": "A1-A3"}, {"value": "5.16918690322743E-5", "module": "A5", "scenario": "Entsorgung Verpackung"}, {"value": "0.00205785707543751", "module": "C2"}, {"value": "0.00496193881540385", "module": "C3"}, {"value": "-0.09380787187088023", "module": "D", "scenario": "energetisch"}, {"value": "-0.03314627549375542", "module": "D", "scenario": "stofflich"}, {"name": "referenceToUnitGroupDataSet", "value": {"shortDescription": [{"value": "kg N eqv."}], "type": "unit group data set", "refObjectId": "d05bb823-ecdf-4686-8c40-bf1d9257859f", "uri": "../unitgroups/d05bb823-ecdf-4686-8c40-bf1d9257859f"}}]}}, {"referenceToLCIAMethodDataSet": {"shortDescription": [{"value": "Eutrophication potential - terrestrial (EP-terrestrial)", "lang": "en"}, {"value": "Eutrophierungspotenzial - Land (EP-terrestrial)", "lang": "de"}], "type": "LCIA method data set", "refObjectId": "b5c614d2-def3-11e6-bf01-fe55135034f3", "version": "01.02.010", "uri": "http://lca.jrc.ec.europa.eu/lcainfohub/datasets/elcd/lciamethods/40054970-5936-477c-9bec-29fa23b1cb77.xml"}, "meanAmount": 0.0, "other": {"anies": [{"value": "1.6535610924946111", "module": "A1"}, {"value": "0.9013753472670475", "module": "A2"}, {"value": "1.6303319789078976", "module": "A3"}, {"value": "4.185268418669557", "module": "A1-A3"}, {"value": "0.00139278136191296", "module": "A5", "scenario": "Entsorgung Verpackung"}, {"value": "0.0228173002500204", "module": "C2"}, {"value": "0.051253487395375", "module": "C3"}, {"value": "-0.6886053259968676", "module": "D", "scenario": "energetisch"}, {"value": "-0.3652206845432795", "module": "D", "scenario": "stofflich"}, {"name": "referenceToUnitGroupDataSet", "value": {"shortDescription": [{"value": "mol N eqv."}], "type": "unit group data set", "refObjectId": "71b4d617-0ec9-4d3f-b65e-e438940c2401", "uri": "../unitgroups/71b4d617-0ec9-4d3f-b65e-e438940c2401"}}]}}, {"referenceToLCIAMethodDataSet": {"shortDescription": [{"value": "Versauerungspotenzial, kumulierte Überschreitung (AP)", "lang": "en"}, {"value": "Bildungspotenzial für troposphärisches Ozon (POCP)", "lang": "de"}], "type": "LCIA method data set", "refObjectId": "b5c610fe-def3-11e6-bf01-fe55135034f3", "version": "02.00.014", "uri": "http://lca.jrc.ec.europa.eu/lcainfohub/datasets/elcd/lciamethods/ec7836be-83eb-41da-bcda-1a6a3fe2d149.xml"}, "meanAmount": 0.0, "other": {"anies": [{"value": "0.4084775924878744", "module": "A1"}, {"value": "0.15277866405064208", "module": "A2"}, {"value": "0.43108499630155805", "module": "A3"}, {"value": "0.9923412528400746", "module": "A1-A3"}, {"value": "1.34279069309139E-4", "module": "A5", "scenario": "Entsorgung Verpackung"}, {"value": "0.00387225996604887", "module": "C2"}, {"value": "0.0118762981350359", "module": "C3"}, {"value": "-0.2222599160772232", "module": "D", "scenario": "energetisch"}, {"value": "-0.08395585225079198", "module": "D", "scenario": "stofflich"}, {"name": "referenceToUnitGroupDataSet", "value": {"shortDescription": [{"value": "kg NMVOC eqv."}], "type": "unit group data set", "refObjectId": "d27c25f8-fbc1-44c6-b47b-4adbae4199c6", "uri": "../unitgroups/d27c25f8-fbc1-44c6-b47b-4adbae4199c6"}}]}}, {"referenceToLCIAMethodDataSet": {"shortDescription": [{"value": "Abiotic depletion potential - non-fossil resources (ADPE)", "lang": "en"}, {"value": "Potenzial für die Verknappung abiotischer Ressourcen – nicht fossile Ressourcen (ADPE)", "lang": "de"}], "type": "LCIA method data set", "refObjectId": "b2ad6494-c78d-11e6-9d9d-cec0c932ce01", "version": "01.00.011"}, "meanAmount": 0.0, "other": {"anies": [{"value": "2.920704637318186E-5", "module": "A1"}, {"value": "1.7813534959648618E-6", "module": "A2"}, {"value": "1.3458237835082717E-5", "module": "A3"}, {"value": "4.444663770422944E-5", "module": "A1-A3"}, {"value": "1.34281756466364E-9", "module": "A5", "scenario": "Entsorgung Verpackung"}, {"value": "4.41042557642647E-8", "module": "C2"}, {"value": "1.8063451141119E-6", "module": "C3"}, {"value": "-4.0574346219376744E-5", "module": "D", "scenario": "energetisch"}, {"value": "-9.988158570029768E-7", "module": "D", "scenario": "stofflich"}, {"name": "referenceToUnitGroupDataSet", "value": {"shortDescription": [{"value": "kg Sb-Äqv."}], "type": "unit group data set", "refObjectId": "54ccd2d9-a32a-4fc2-923d-f2c8c93e89d4", "uri": "../unitgroups/54ccd2d9-a32a-4fc2-923d-f2c8c93e89d4"}}]}}, {"referenceToLCIAMethodDataSet": {"shortDescription": [{"value": "Abiotic depletion potential - fossil resources (ADPF)", "lang": "en"}, {"value": "Potenzial für die Verknappung abiotischer Ressourcen – fossile Brennstoffe (ADPF)", "lang": "de"}], "type": "LCIA method data set", "refObjectId": "b2ad6110-c78d-11e6-9d9d-cec0c932ce01", "version": "01.00.011"}, "meanAmount": 0.0, "other": {"anies": [{"value": "908.3430811561137", "module": "A1"}, {"value": "367.92514316901384", "module": "A2"}, {"value": "928.8257178619742", "module": "A3"}, {"value": "2205.0939421871017", "module": "A1-A3"}, {"value": "0.307808443835602", "module": "A5", "scenario": "Entsorgung Verpackung"}, {"value": "9.29744150049595", "module": "C2"}, {"value": "139.662614537349", "module": "C3"}, {"value": "-4213.574088077632", "module": "D", "scenario": "energetisch"}, {"value": "-151.98667835319242", "module": "D", "scenario": "stofflich"}, {"name": "referenceToUnitGroupDataSet", "value": {"shortDescription": [{"value": "MJ"}], "type": "unit group data set", "refObjectId": "93a60a57-a3c8-11da-a746-0800200c9a66", "uri": "../unitgroups/93a60a57-a3c8-11da-a746-0800200c9a66"}}]}}, {"referenceToLCIAMethodDataSet": {"shortDescription": [{"value": "Water (user) deprivation potential (WDP)", "lang": "en"}, {"value": "Wasser-Entzugspotenzial (Benutzer) (WDP)", "lang": "de"}], "type": "LCIA method data set", "refObjectId": "b2ad66ce-c78d-11e6-9d9d-cec0c932ce01", "version": "03.00.015"}, "meanAmount": 0.0, "other": {"anies": [{"value": "0.1485406507823704", "module": "A1"}, {"value": "0.02740264524214419", "module": "A2"}, {"value": "0.25711676363635", "module": "A3"}, {"value": "0.4330600596608646", "module": "A1-A3"}, {"value": "0.00397374631663949", "module": "A5", "scenario": "Entsorgung Verpackung"}, {"value": "7.25105792993116E-4", "module": "C2"}, {"value": "0.0460593600990649", "module": "C3"}, {"value": "0.926665205404396", "module": "D", "scenario": "energetisch"}, {"value": "-0.01735918861460875", "module": "D", "scenario": "stofflich"}, {"name": "referenceToUnitGroupDataSet", "value": {"shortDescription": [{"value": "m3 world eqv."}], "type": "unit group data set", "refObjectId": "6ae2df01-888e-46c8-b17d-49fa3869b476", "uri": "../unitgroups/6ae2df01-888e-46c8-b17d-49fa3869b476"}}]}}, {"referenceToLCIAMethodDataSet": {"shortDescription": [{"value": "Global Warming Potential - land use and land use change (GWP-luluc)", "lang": "en"}, {"value": "Globales Erwärmungspotenzial - luluc (GWP-luluc)", "lang": "de"}], "type": "LCIA method data set", "refObjectId": "4331bbdb-978a-490d-8707-eeb047f01a55", "version": "01.00.006"}, "meanAmount": 0.0, "other": {"anies": [{"module": "A1"}, {"module": "A2"}, {"module": "A3"}, {"module": "A1-A3"}, {"module": "A5", "scenario": "Entsorgung Verpackung"}, {"module": "C2"}, {"module": "C3"}, {"module": "D", "scenario": "energetisch"}, {"module": "D", "scenario": "stofflich"}, {"name": "referenceToUnitGroupDataSet", "value": {"shortDescription": [{"value": "kg CO2-Äqv."}], "type": "unit group data set", "refObjectId": "1ebf3012-d0db-4de2-aefd-ef30cedb0be1", "uri": "../unitgroups/1ebf3012-d0db-4de2-aefd-ef30cedb0be1"}}]}}, {"referenceToLCIAMethodDataSet": {"shortDescription": [{"value": "Potential incidence of disease due to PM emissions (PM)", "lang": "en"}, {"value": "Potenzielles Auftreten von Krankheiten aufgrund von Feinstaubemissionen (PM)", "lang": "de"}], "type": "LCIA method data set", "refObjectId": "b5c602c6-def3-11e6-bf01-fe55135034f3", "version": "02.00.012", "uri": "http://lca.jrc.ec.europa.eu/lcainfohub/datasets/elcd/lciamethods/72ce3013-f678-4c6a-935b-f4752ff8901b.xml"}, "meanAmount": 0.0, "other": {"anies": [{"module": "A1"}, {"module": "A2"}, {"module": "A3"}, {"module": "A1-A3"}, {"module": "A5", "scenario": "Entsorgung Verpackung"}, {"module": "C2"}, {"module": "C3"}, {"module": "D", "scenario": "energetisch"}, {"module": "D", "scenario": "stofflich"}, {"name": "referenceToUnitGroupDataSet", "value": {"shortDescription": [{"value": "disease incidence"}], "type": "unit group data set", "refObjectId": "3883559b-648f-4afc-8ba2-0bd24f3affa3", "uri": "../unitgroups/3883559b-648f-4afc-8ba2-0bd24f3affa3"}}]}}, {"referenceToLCIAMethodDataSet": {"shortDescription": [{"value": "Potential Human exposure efficiency relative to U235 (IRP)", "lang": "en"}, {"value": "Potenzielle Wirkung durch Exposition des Menschen mit U235 (IRP)", "lang": "de"}], "type": "LCIA method data set", "refObjectId": "b5c632be-def3-11e6-bf01-fe55135034f3", "version": "01.00.012", "uri": "http://lca.jrc.ec.europa.eu/lcainfohub/datasets/elcd/lciamethods/a6f4cbc8-5388-44d6-9a67-53d05684f93e.xml"}, "meanAmount": 0.0, "other": {"anies": [{"module": "A1"}, {"module": "A2"}, {"module": "A3"}, {"module": "A1-A3"}, {"module": "A5", "scenario": "Entsorgung Verpackung"}, {"module": "C2"}, {"module": "C3"}, {"module": "D", "scenario": "energetisch"}, {"module": "D", "scenario": "stofflich"}, {"name": "referenceToUnitGroupDataSet", "value": {"shortDescription": [{"value": "kBq U235 eqv."}], "type": "unit group data set", "refObjectId": "456b05bf-1415-44a9-9993-02452f554c09", "uri": "../unitgroups/456b05bf-1415-44a9-9993-02452f554c09"}}]}}, {"referenceToLCIAMethodDataSet": {"shortDescription": [{"value": "Potential Comparative Toxic Unit for ecosystems (ETP-fw)", "lang": "en"}, {"value": "Potenzielle Toxizitätsvergleichseinheit für Ökosysteme (ETP-fw)", "lang": "de"}], "type": "LCIA method data set", "refObjectId": "ee1082d1-b0f7-43ca-a1f0-21e2a4a74511", "version": "01.00.003", "uri": "http://lca.jrc.ec.europa.eu/lcainfohub/datasets/elcd/lciamethods/ee1082d1-b0f7-43ca-a1f0-21e2a4a74511.xml"}, "meanAmount": 0.0, "other": {"anies": [{"module": "A1"}, {"module": "A2"}, {"module": "A3"}, {"module": "A1-A3"}, {"module": "A5", "scenario": "Entsorgung Verpackung"}, {"module": "C2"}, {"module": "C3"}, {"module": "D", "scenario": "energetisch"}, {"module": "D", "scenario": "stofflich"}, {"name": "referenceToUnitGroupDataSet", "value": {"shortDescription": [{"value": "CTUe"}], "type": "unit group data set", "refObjectId": "aa959ded-f1eb-4efb-9c5c-2d60be36b3e6", "uri": "../unitgroups/aa959ded-f1eb-4efb-9c5c-2d60be36b3e6"}}]}}, {"referenceToLCIAMethodDataSet": {"shortDescription": [{"value": "Potential Comparative Toxic Unit for humans - cancer effects (HTP-c)", "lang": "en"}, {"value": "Potenzielle Toxizitätsvergleichseinheit für den Menschen - kanzerogene Wirkung (HTP-c)", "lang": "de"}], "type": "LCIA method data set", "refObjectId": "2299222a-bbd8-474f-9d4f-4dd1f18aea7c", "version": "01.00.004", "uri": "http://lca.jrc.ec.europa.eu/lcainfohub/datasets/elcd/lciamethods/2299222a-bbd8-474f-9d4f-4dd1f18aea7c.xml"}, "meanAmount": 0.0, "other": {"anies": [{"module": "A1"}, {"module": "A2"}, {"module": "A3"}, {"module": "A1-A3"}, {"module": "A5", "scenario": "Entsorgung Verpackung"}, {"module": "C2"}, {"module": "C3"}, {"module": "D", "scenario": "energetisch"}, {"module": "D", "scenario": "stofflich"}, {"name": "referenceToUnitGroupDataSet", "value": {"shortDescription": [{"value": "CTUh"}], "type": "unit group data set", "refObjectId": "d4c9523e-2d7e-49fd-8469-998f547d3a70", "uri": "../unitgroups/d4c9523e-2d7e-49fd-8469-998f547d3a70"}}]}}, {"referenceToLCIAMethodDataSet": {"shortDescription": [{"value": "Potential Comparative Toxic Unit for humans - non-cancer effects (HTP-nc)", "lang": "en"}, {"value": "Potenzielle Toxizitätsvergleichseinheit für den Menschen - nicht kanzerogene Wirkung (HTP-nc)", "lang": "de"}], "type": "LCIA method data set", "refObjectId": "3af763a5-b7a1-48c9-9cee-1f223481fcef", "version": "01.00.003", "uri": "http://lca.jrc.ec.europa.eu/lcainfohub/datasets/elcd/lciamethods/3af763a5-b7a1-48c9-9cee-1f223481fcef.xml"}, "meanAmount": 0.0, "other": {"anies": [{"module": "A1"}, {"module": "A2"}, {"module": "A3"}, {"module": "A1-A3"}, {"module": "A5", "scenario": "Entsorgung Verpackung"}, {"module": "C2"}, {"module": "C3"}, {"module": "D", "scenario": "energetisch"}, {"module": "D", "scenario": "stofflich"}, {"name": "referenceToUnitGroupDataSet", "value": {"shortDescription": [{"value": "CTUh"}], "type": "unit group data set", "refObjectId": "d4c9523e-2d7e-49fd-8469-998f547d3a70", "uri": "../unitgroups/d4c9523e-2d7e-49fd-8469-998f547d3a70"}}]}}, {"referenceToLCIAMethodDataSet": {"shortDescription": [{"value": "Potential Soil quality index (SQP)", "lang": "en"}, {"value": "Potenzieller Bodenqualitätsindex (SQP)", "lang": "de"}], "type": "LCIA method data set", "refObjectId": "b2ad6890-c78d-11e6-9d9d-cec0c932ce01", "version": "01.00.011"}, "meanAmount": 0.0, "other": {"anies": [{"module": "A1"}, {"module": "A2"}, {"module": "A3"}, {"module": "A1-A3"}, {"module": "A5", "scenario": "Entsorgung Verpackung"}, {"module": "C2"}, {"module": "C3"}, {"module": "D", "scenario": "energetisch"}, {"module": "D", "scenario": "stofflich"}, {"name": "referenceToUnitGroupDataSet", "value": {"shortDescription": [{"value": "dimensionless"}], "type": "unit group data set", "refObjectId": "f130951c-e67f-4f7f-8dd4-665de3974e18", "uri": "../unitgroups/f130951c-e67f-4f7f-8dd4-665de3974e18"}}]}}]}, "otherAttributes": {"{http://www.okworx.com/ILCD/Extensions/2018/Profile}profile": "EN_15804_A2", "{http://www.indata.network/EPD/2019}epd-version": "1.2"}, "version": "1.1"}