{"processInformation": {"dataSetInformation": {"UUID": "cddad814-59d9-4e84-9fa9-8b93b17cda9b", "name": {"baseName": [{"value": "JACKODUR EVO", "lang": "en"}, {"value": "JACKODUR EVO", "lang": "de"}], "functionalUnitFlowProperties": [{"lang": "en"}]}, "classificationInformation": {"classification": [{"class": [{"value": "Dämmstoffe", "level": 0, "classId": "2"}, {"value": "Extrudiertes Polystyrol (XPS)", "level": 1, "classId": "2.3"}, {"value": "XPS weiß", "level": 2, "classId": "2.3.01"}], "name": "OEKOBAU.DAT"}, {"class": [{"value": "02 Building products", "level": 0}, {"value": "Thermal insulation products", "level": 1}, {"value": "Insulating materials made of foam plastics", "level": 2}], "name": "IBUCategories"}]}, "generalComment": [{"value": "JACKODUR EVO is an extruded polystyrene foam (XPS) produced according to EN 13164 and available in board shape with a density range from 28 to 40 kg/m3, 34.37 kg/m3 in average (measured). It has specifically low values of thermal conductivity. The boards can be delivered in various compressive strength values from 300 to 700 kPa. To meet the need of various applications the boards are produced with different surfaces: with the extrusion skin, planed, grooved or with thermal embossing. JACKODUR EVO boards are supplied with different edge treatments such as butt edge, ship-lap and tongue and groove. The EPD is related to an unlaminated product only; lamination and additional product treatment are not considered.", "lang": "en"}, {"value": "XPS mit teilweise recyceltem Materialeinsatz", "lang": "de"}], "other": {"anies": [{"scenario": [{"description": [{"value": "100 % energy recovery", "lang": "en"}, {"value": "100% thermische Weiterverwendung (Verbrennung)", "lang": "de"}], "name": "S1", "default": true}, {"description": [{"value": "100% recycling", "lang": "en"}, {"value": "100% Recycling", "lang": "de"}], "name": "S2"}, {"description": [{"value": "100% landfilling", "lang": "en"}, {"value": "100% Deponie", "lang": "de"}], "name": "S3"}]}]}}, "quantitativeReference": {"referenceToReferenceFlow": [0]}, "time": {"referenceYear": 2023, "dataSetValidUntil": 2028, "other": {"anies": [{"name": "publicationDateOfEPD", "value": 1702944000000}]}}, "geography": {"locationOfOperationSupplyOrProduction": {"location": "RER"}}, "technology": {"technologyDescriptionAndIncludedProcesses": [{"value": "JACKODUR EVO is an extruded polystyrene foam (XPS) produced according to EN 13164 and available in board shape with a density range from 28 to 40 kg/m3, 34.37 kg/m3in average (measured). It has specifically low values of thermal conductivity. The boards can be delivered in various compressive strength values from 300 to 700 kPa. To meet the need of various applications the boards are produced with different surfaces: with the extrusion skin, planed, grooved or with thermal embossing. JACKODUR EVO boards are supplied with different edge treatments such as butt edge, ship-lap and tongue and groove. The EPD is related to an unlaminated product only; lamination and additional product treatment are not considered. JACKODUR EVO is made of polystyrene (90 to 95% by weight – CAS 9003-53-6), blown with carbon dioxide (CAS 124-38-9) and halogen-free co-blowing agents altogether up to 8% by weight. More than 30% of the polystyrene is secondary polystyrene (internally recycled and post consumer recycled material), the amount of post consumer recycled material is higher than 5% of the polystyrene. \nTechnical data: \nAcoustic properties are not relevant for JACKODUR EVO. For fire performance, these products achieve the fire classification Euroclass E according to EN 13501-1. \nDeclared unit: \nThe declared unit is 1 m3 of the XPS board, JACKODUR EVO.", "lang": "en"}, {"value": "XPS wird in einem kontinuierlichen EXtrusionsprozess mit Strom als Hauptenergieträger hergestellt.\nPolystyrol-Granulat und recyceltes Polystyrol wird zusammen mit den Hilfsstoffen im Extruder unter hohem Druck aufgeschmolzen. Das Treibmittel wird der Schmelze hinzugegeben und in ihr gelöst. Die Schmelze wird durch eine Breitschlitzdüse ausgetragen. Durch den\ndabei abfallenden Gegendruck schäumt das\nTreibmittel die Schmelze auf, kühlt diese dabei ab und das Polystyrol verfestigt sich. Es entsteht ein endloser Strang aus homogenem und geschlossenzelligem Polystyrolhartschaum. Dieser wird weiter abgekühlt und anschließend dimensioniert, besäumt und eventuell in der Oberfläche modifiziert.  XPS aus Produktionsabschnitten und Produktionsausschuss wird direkt in den Produktionen recycliert und wieder zur  roduktion von XPS eingesetzt.\nPolystyrol ist ein thermoplastisches Material und\ndeshalb kann Abfall vor Gebrauch (industrieller Abfall) einfach und kostengünstig durch Aufschmelzen recycliert werden.\nDie meisten XPS-Abfälle, die bei der Herstellung\nanfallen, werden gemahlen und in einer separaten Linie extrudiert. Das daraus resultierende Recyclat wird dann im Produktionsprozess von XPS verwendet. \nTechnische Daten: \nJACKODUR EVO ist ein extrudierter Polystyrolschaum (XPS), hergestellt nach EN 13164 und erhältlich in Plattenform mit einem Dichtebereich von 28 bis 40 kg/m3, durchschnittlich 34,37 kg/m3 (gemessen). Es weist besonders niedrige Werte der Wärmeleitfähigkeit auf. Die Platten können in verschiedenen Druckfestigkeitswerten von 300 bis 700 kPa geliefert werden. Um den Anforderungen unterschiedlicher Anwendungen gerecht zu werden, werden die Platten mit unterschiedlichen Oberflächen hergestellt: mit Extrusionshaut, gehobelt, gerillt oder mit Thermoprägung. JACKODUR EVO-Platten werden mit verschiedenen Kantenbehandlungen wie Stoßkante, Überlappung und Nut und Feder geliefert. Die EPD bezieht sich nur auf ein unlaminiertes Produkt; Laminierung und zusätzliche Produktbehandlung sind nicht berücksichtigt. \nDeklarierte Einheit: \n1 m3", "lang": "de"}], "technologicalApplicability": [{"value": "The variety of the performance properties of JACKODUR EVO make it suitable for use in a large number of applications such as: perimeter insulation, inverted roof insulation, insulation of pitched roofs, floor insulation including insulation of highly loaded industrial floors, insulation of thermal bridges for exterior walls, External Thermal Insulation Composite Systems (ETICS), insulation of cavity walls, agricultural building ceiling insulation, prefabricated elements e.g. building sandwich panels, insulation for building equipment and industrial installations (pipe sections, ...)", "lang": "en"}, {"value": "Die vielfältigen Leistungseigenschaften von JACKODUR EVO ermöglichen den Einsatz in einer Vielzahl von Anwendungen wie: Perimeterdämmung, Umkehrdachdämmung, Dämmung von Steildächern, Bodendämmung einschließlich Dämmung hochbelasteter Industrieböden, Dämmung von Wärmebrücken Außenwände, Wärmedämmverbundsysteme (WDVS), Dämmung von Hohlwänden, Deckendämmung landwirtschaftlicher Gebäude, vorgefertigte Elemente z.B. Bausandwichplatten, Isolierung für Gebäudeausrüstung und Industrieanlagen (Rohrabschnitte, ...)", "lang": "de"}]}}, "modellingAndValidation": {"LCIMethodAndAllocation": {"typeOfDataSet": "EPD", "referenceToLCAMethodDetails": [{"shortDescription": [{"value": "Insulating materials made of foam plastics.pdf", "lang": "en"}], "type": "source data set", "refObjectId": "bf67f9a9-ad54-482a-87d8-fe0312018f12"}], "other": {"anies": [{"name": "subType", "value": "specific dataset"}]}}, "dataSourcesTreatmentAndRepresentativeness": {"referenceToDataSource": [{"shortDescription": [{"value": "GaBi Database (all versions)", "lang": "en"}], "type": "source data set", "refObjectId": "28d74cc0-db8b-4d7e-bc44-5f6d56ce0c4a"}, {"shortDescription": [{"value": "Sphera MLC (fka GaBi) CUP 2023.01", "lang": "en"}], "type": "source data set", "refObjectId": "6bcd5bfa-3623-48ab-a52b-6d5be8db82ed"}], "useAdviceForDataSet": [{"value": "Scope: \nJACKON Insulation, as data provider, produces the extruded polystyrene foam boards JACKODUR EVO containing CO2 as blowing agent and use more than 5% post consumer recycled polystyrene (rGPPS) content plus approximately 28% reclaimed/recovered content via internal recycling. The data have been provided by one factory in Arendsee/Germany for the second half year 2022. \nSystem boundary: \nType of EPD according to EN 15804: \"cradle to gate\nwith options, modules C1–C4, and module D\". The following modules are declared: A1–A3, C, D and additional modules: A4 + A5.\n\nModules A1-A3\nThe product stage includes:\nRaw material supply (A1) comprises the production of virgin and recycled polystyrene granulate, blowing and co-blowing agents as well as flame retardants.\nThe transport to the manufacturer is considered in module A2.\nThe manufacturing of the XPS board (A3) comprises the provision of all materials, products and energy, as well as waste processing up to the end-of-waste state, including packaging of the product and the internal recycling process of the foam scrap.\nModules A4-A5\nThe construction process stage includes:\nTransport to the construction site (A4) \nTreatment of packaging material (A5) with benefit for potential avoided burdens due to energy substitution of electricity and thermal energy generation are declared in module D (D/1, D/2, and D/3).Modules C1-C4 and D\nThe end-of-life stage includes:\nManual dismantling (C1) \nTransport to EoL (C2) \nWaste processing & disposal (C) with three 100 % scenarios (scenario 1: thermal treatment (C3/1); scenario 2: recycling(C3/2); scenario 3: landfill (C4/3)). \nThe resulting potential benefits for thermal and electrical energy from energy substitution from incineration (packaging material in A5 and the product in C3/1) and from recycling (C3/2) material benefit for the recycled material are considered in modules D/1 and D/2, respectively. This affects only the rate of primary materials (no secondary materials). The benefits in D/3 solely account for the avoided burdens calculated by the inversion of the electricity grid mix and thermal energy from natural gas during packaging treatment (A5). This is considered under European conditions.", "lang": "en"}, {"value": "Gültigkeitsbereich: \nJACKON Insulation produziert als Datenlieferant die extrudierten Polystyrolschaumplatten JACKODUR EVO mit CO2 als Treibmittel und verwendet mehr als 30 % Sekundärpolystyrol. Die Daten wurden von einem Werk in Arendsee/Deutschland für das zweite Halbjahr 2022 bereitgestellt. \nSystemgrenze: \nArt der EPD nach EN 15804: „Cradle to Gate“.\nmit Optionen, Modulen C1–C4 und Modul D“. Folgende Module sind deklariert: A1–A3, C, D und Zusatzmodule: A4 + A5.", "lang": "de"}], "other": {"anies": [{"name": "referenceToOriginalEPD", "value": {"shortDescription": {"value": "JACKODUR EVO.pdf", "defaultValue": "JACKODUR EVO.pdf", "lstrings": [{"lang": "en", "value": "JACKODUR EVO.pdf"}]}, "type": "source data set", "uuid": {"uuid": "0ba81f25-aa8a-4201-a152-421165cc2f30"}, "refObjectId": "0ba81f25-aa8a-4201-a152-421165cc2f30", "resourceURLs": ["https://oekobaudat.de/OEKOBAU.DAT/resource/sources/0ba81f25-aa8a-4201-a152-421165cc2f30/JACKODUR_EVO_17946.pdf?version=00.01.000"]}}]}}, "validation": {"review": [{"referenceToNameOfReviewerAndInstitution": [{"shortDescription": [{"value": "Institut Bauen und Umwelt e. V.", "lang": "en"}], "type": "contact data set", "refObjectId": "d111dbec-b024-4be5-86c5-752d6eb2cf95", "uri": "../contacts/d111dbec-b024-4be5-86c5-752d6eb2cf95.xml"}], "type": "Accredited third party review"}]}, "complianceDeclarations": {"compliance": [{"referenceToComplianceSystem": {"shortDescription": [{"value": "DIN EN 15804+A2", "lang": "en"}], "type": "source data set", "refObjectId": "c0016b33-8cf7-415c-ac6e-deba0d21440d", "uri": "../sources/c0016b33-8cf7-415c-ac6e-deba0d21440d.xml"}}, {"referenceToComplianceSystem": {"shortDescription": [{"value": "ISO 14025", "lang": "en"}], "type": "source data set", "refObjectId": "4f2eb655-6e44-4874-a95a-e28f5442cd4d", "uri": "../sources/4f2eb655-6e44-4874-a95a-e28f5442cd4d.xml"}}]}}, "administrativeInformation": {"commissionerAndGoal": {"referenceToCommissioner": [{"shortDescription": [{"value": "JACKON Insulation GmbH", "lang": "en"}], "type": "contact data set", "refObjectId": "535c67fe-b4a8-4cf0-b3e4-bd91ca22b281", "uri": "../contacts/535c67fe-b4a8-4cf0-b3e4-bd91ca22b281.xml"}]}, "dataGenerator": {"referenceToPersonOrEntityGeneratingTheDataSet": [{"shortDescription": [{"value": "Sphera Solutions GmbH", "lang": "en"}], "type": "contact data set", "refObjectId": "623edf96-39d1-4e6f-9892-674c7228546b", "uri": "../contacts/623edf96-39d1-4e6f-9892-674c7228546b.xml"}]}, "dataEntryBy": {"timeStamp": 1702944000000, "referenceToDataSetFormat": [{"shortDescription": [{"value": "ILCD Format", "lang": "en"}], "type": "source data set", "refObjectId": "a97a0155-0234-4b87-b4ce-a45da52f2a40", "uri": "../sources/a97a0155-0234-4b87-b4ce-a45da52f2a40.xml"}, {"shortDescription": [{"value": "EPD-Datenformaterweiterungen v1.2", "lang": "de"}, {"value": "EPD Data Format Extensions v1.2", "lang": "en"}], "type": "source data set", "refObjectId": "a29449fd-aa2f-4de8-b5d7-4b06b43c6fde", "uri": "../sources/a29449fd-aa2f-4de8-b5d7-4b06b43c6fde.xml"}]}, "publicationAndOwnership": {"dataSetVersion": "00.03.000", "referenceToRegistrationAuthority": {"shortDescription": [{"value": "Institut Bauen und Umwelt e. V.", "lang": "en"}], "type": "contact data set", "refObjectId": "d111dbec-b024-4be5-86c5-752d6eb2cf95", "uri": "../contacts/d111dbec-b024-4be5-86c5-752d6eb2cf95.xml"}, "registrationNumber": "EPD-JAC-20220371-CBA1-EN", "referenceToOwnershipOfDataSet": {"shortDescription": [{"value": "JACKON Insulation GmbH", "lang": "en"}], "type": "contact data set", "refObjectId": "535c67fe-b4a8-4cf0-b3e4-bd91ca22b281", "uri": "../contacts/535c67fe-b4a8-4cf0-b3e4-bd91ca22b281.xml"}, "copyright": true, "licenseType": "Free of charge for all users and uses", "accessRestrictions": [{"value": "None", "lang": "en"}], "other": {"anies": [{"name": "referenceToPublisher", "value": {"shortDescription": [{"value": "Institut Bauen und Umwelt e. V.", "lang": "en"}], "type": "contact data set", "refObjectId": "d111dbec-b024-4be5-86c5-752d6eb2cf95", "uri": "../contacts/d111dbec-b024-4be5-86c5-752d6eb2cf95.xml"}}]}}}, "exchanges": {"exchange": [{"dataSetInternalID": 0, "referenceToFlowDataSet": {"shortDescription": [{"value": "JACKODUR EVO (JACKODUR EVO)", "lang": "en"}], "type": "flow data set", "refObjectId": "2837270e-5244-9dbc-bc86-8c11a56afcb4", "uri": "../flows/2837270e-5244-9dbc-bc86-8c11a56afcb4.xml"}, "meanAmount": 1.0, "referencesToDataSource": {}, "referenceFlow": true, "resolvedFlowVersion": "00.02.000", "resultingflowAmount": 1.0, "flowProperties": [{"name": [{"lang": "en", "value": "Volume"}, {"lang": "de", "value": "Volumen"}], "uuid": "93a60a56-a3c8-22da-a746-0800200c9a66", "referenceFlowProperty": true, "meanValue": 1.0, "referenceUnit": "m3", "unitGroupUUID": "cd950537-0a98-4044-9ba7-9f9a68d0a504"}], "materialProperties": [{"name": "gross density", "value": "34.37", "unit": "kg/m^3", "unitDescription": "kilograms per cubic metre"}], "typeOfFlow": "Product flow", "classification": {"classHierarchy": "Dämmstoffe / Extrudiertes Polystyrol (XPS) / XPS weiß", "name": "OEKOBAU.DAT"}}, {"dataSetInternalID": 1, "referenceToFlowDataSet": {"shortDescription": [{"value": "Renewable primary energy as energy carrier (PERE)", "lang": "en"}, {"value": "Erneuerbare Primärenergie als Energieträger (PERE)", "lang": "de"}], "type": "flow data set", "refObjectId": "20f32be5-0398-4288-9b6d-accddd195317", "uri": "../flows/20f32be5-0398-4288-9b6d-accddd195317.xml"}, "exchange direction": "INPUT", "other": {"anies": [{"name": "referenceToUnitGroupDataSet", "value": {"shortDescription": [{"value": "MJ", "lang": "en"}], "type": "unit group data set", "refObjectId": "93a60a57-a3c8-11da-a746-0800200c9a66", "uri": "../unitgroups/93a60a57-a3c8-11da-a746-0800200c9a66.xml"}}, {"value": "77.1962673851304", "module": "A1-A3"}, {"value": "1.24401449946213", "module": "A4"}, {"value": "0.0624677047785322", "module": "A5"}, {"value": "0", "module": "C1"}, {"value": "0.122088970464902", "module": "C2"}, {"value": "3.37450360498103", "module": "C3", "scenario": "S1"}, {"value": "54.1338776098969", "module": "C3", "scenario": "S2"}, {"value": "3.18384678909202", "module": "C4"}, {"value": "-70.8789729163046", "module": "D", "scenario": "S1"}, {"value": "-46.2119863964364", "module": "D", "scenario": "S2"}, {"value": "-1.50805084314907", "module": "D", "scenario": "S3"}]}, "resolvedFlowVersion": "38.00.000", "flowProperties": [], "typeOfFlow": "Other flow", "classification": {"classHierarchy": "Quantities", "name": "GaBiCategories"}}, {"dataSetInternalID": 2, "referenceToFlowDataSet": {"shortDescription": [{"value": "Renewable primary energy resources as material utilization (PERM)", "lang": "en"}, {"value": "Erneuerbare Primärenergie zur stofflichen Nutzung (PERM)", "lang": "de"}], "type": "flow data set", "refObjectId": "fb3ec0de-548d-4508-aea5-00b73bf6f702", "uri": "../flows/fb3ec0de-548d-4508-aea5-00b73bf6f702.xml"}, "exchange direction": "INPUT", "other": {"anies": [{"name": "referenceToUnitGroupDataSet", "value": {"shortDescription": [{"value": "MJ", "lang": "en"}], "type": "unit group data set", "refObjectId": "93a60a57-a3c8-11da-a746-0800200c9a66", "uri": "../unitgroups/93a60a57-a3c8-11da-a746-0800200c9a66.xml"}}, {"value": "0", "module": "A1-A3"}, {"value": "0", "module": "A4"}, {"value": "0", "module": "A5"}, {"value": "0", "module": "C1"}, {"value": "0", "module": "C2"}, {"value": "0", "module": "C3", "scenario": "S1"}, {"value": "0", "module": "C3", "scenario": "S2"}, {"value": "0", "module": "C4"}, {"value": "0", "module": "D", "scenario": "S1"}, {"value": "0", "module": "D", "scenario": "S2"}, {"value": "0", "module": "D", "scenario": "S3"}]}, "resolvedFlowVersion": "38.00.000", "flowProperties": [], "typeOfFlow": "Other flow", "classification": {"classHierarchy": "Quantities", "name": "GaBiCategories"}}, {"dataSetInternalID": 3, "referenceToFlowDataSet": {"shortDescription": [{"value": "Total use of renewable primary energy resources (PERT)", "lang": "en"}, {"value": "Total erneuerbare Primärenergie (PERT)", "lang": "de"}], "type": "flow data set", "refObjectId": "53f97275-fa8a-4cdd-9024-65936002acd0", "uri": "../flows/53f97275-fa8a-4cdd-9024-65936002acd0.xml"}, "exchange direction": "INPUT", "other": {"anies": [{"name": "referenceToUnitGroupDataSet", "value": {"shortDescription": [{"value": "MJ", "lang": "en"}], "type": "unit group data set", "refObjectId": "93a60a57-a3c8-11da-a746-0800200c9a66", "uri": "../unitgroups/93a60a57-a3c8-11da-a746-0800200c9a66.xml"}}, {"value": "77.1962673851304", "module": "A1-A3"}, {"value": "1.24401449946213", "module": "A4"}, {"value": "0.0624677047785322", "module": "A5"}, {"value": "0", "module": "C1"}, {"value": "0.122088970464902", "module": "C2"}, {"value": "3.37450360498103", "module": "C3", "scenario": "S1"}, {"value": "54.1338776098969", "module": "C3", "scenario": "S2"}, {"value": "3.18384678909202", "module": "C4"}, {"value": "-70.8789729163046", "module": "D", "scenario": "S1"}, {"value": "-46.2119863964364", "module": "D", "scenario": "S2"}, {"value": "-1.50805084314907", "module": "D", "scenario": "S3"}]}, "resolvedFlowVersion": "38.00.000", "flowProperties": [], "typeOfFlow": "Other flow", "classification": {"classHierarchy": "Quantities / Environmental quantities / EPD EN 15804 / LCI indicators", "name": "GaBiCategories"}}, {"dataSetInternalID": 4, "referenceToFlowDataSet": {"shortDescription": [{"value": "Non renewable primary energy as energy carrier (PENRE)", "lang": "en"}, {"value": "Nicht-erneuerbare Primärenergie als Energieträger (PENRE)", "lang": "de"}], "type": "flow data set", "refObjectId": "ac857178-2b45-46ec-892a-a9a4332f0372", "uri": "../flows/ac857178-2b45-46ec-892a-a9a4332f0372.xml"}, "exchange direction": "INPUT", "other": {"anies": [{"name": "referenceToUnitGroupDataSet", "value": {"shortDescription": [{"value": "MJ", "lang": "en"}], "type": "unit group data set", "refObjectId": "93a60a57-a3c8-11da-a746-0800200c9a66", "uri": "../unitgroups/93a60a57-a3c8-11da-a746-0800200c9a66.xml"}}, {"value": "1599.03574847817", "module": "A1-A3"}, {"value": "17.1587563566984", "module": "A4"}, {"value": "28.8878809192223", "module": "A5"}, {"value": "0", "module": "C1"}, {"value": "1.68397948653586", "module": "C2"}, {"value": "1178.62837332894", "module": "C3", "scenario": "S1"}, {"value": "90.5809707889551", "module": "C3", "scenario": "S2"}, {"value": "35.3042775698384", "module": "C4"}, {"value": "-902.691500702404", "module": "D", "scenario": "S1"}, {"value": "-2257.22310545824", "module": "D", "scenario": "S2"}, {"value": "-19.1932306152495", "module": "D", "scenario": "S3"}]}, "resolvedFlowVersion": "38.00.000", "flowProperties": [], "typeOfFlow": "Other flow", "classification": {"classHierarchy": "Quantities", "name": "GaBiCategories"}}, {"dataSetInternalID": 5, "referenceToFlowDataSet": {"shortDescription": [{"value": "Non renewable primary energy as material utilization (PENRM)", "lang": "en"}, {"value": "Nicht-erneuerbare Primärenergie zur stofflichen Nutzung (PENRM)", "lang": "de"}], "type": "flow data set", "refObjectId": "1421caa0-679d-4bf4-b282-0eb850ccae27", "uri": "../flows/1421caa0-679d-4bf4-b282-0eb850ccae27.xml"}, "exchange direction": "INPUT", "other": {"anies": [{"name": "referenceToUnitGroupDataSet", "value": {"shortDescription": [{"value": "MJ", "lang": "en"}], "type": "unit group data set", "refObjectId": "93a60a57-a3c8-11da-a746-0800200c9a66", "uri": "../unitgroups/93a60a57-a3c8-11da-a746-0800200c9a66.xml"}}, {"value": "1194.244", "module": "A1-A3"}, {"value": "0", "module": "A4"}, {"value": "-28.644", "module": "A5"}, {"value": "0", "module": "C1"}, {"value": "0", "module": "C2"}, {"value": "-1165.6", "module": "C3", "scenario": "S1"}, {"value": "-1165.6", "module": "C3", "scenario": "S2"}, {"value": "0", "module": "C4"}, {"value": "0", "module": "D", "scenario": "S1"}, {"value": "0", "module": "D", "scenario": "S2"}, {"value": "0", "module": "D", "scenario": "S3"}]}, "resolvedFlowVersion": "38.00.000", "flowProperties": [], "typeOfFlow": "Other flow", "classification": {"classHierarchy": "Quantities", "name": "GaBiCategories"}}, {"dataSetInternalID": 6, "referenceToFlowDataSet": {"shortDescription": [{"value": "Total use of non renewable primary energy resources (PENRT)", "lang": "en"}, {"value": "Total nicht erneuerbare Primärenergie (PENRT)", "lang": "de"}], "type": "flow data set", "refObjectId": "06159210-646b-4c8d-8583-da9b3b95a6c1", "uri": "../flows/06159210-646b-4c8d-8583-da9b3b95a6c1.xml"}, "exchange direction": "INPUT", "other": {"anies": [{"name": "referenceToUnitGroupDataSet", "value": {"shortDescription": [{"value": "MJ", "lang": "en"}], "type": "unit group data set", "refObjectId": "93a60a57-a3c8-11da-a746-0800200c9a66", "uri": "../unitgroups/93a60a57-a3c8-11da-a746-0800200c9a66.xml"}}, {"value": "2793.27974847818", "module": "A1-A3"}, {"value": "17.1587563566984", "module": "A4"}, {"value": "0.243880919222352", "module": "A5"}, {"value": "0", "module": "C1"}, {"value": "1.68397948653586", "module": "C2"}, {"value": "13.0283733289375", "module": "C3", "scenario": "S1"}, {"value": "-1075.01902921105", "module": "C3", "scenario": "S2"}, {"value": "35.3042775698386", "module": "C4"}, {"value": "-902.691500702409", "module": "D", "scenario": "S1"}, {"value": "-2257.22310545825", "module": "D", "scenario": "S2"}, {"value": "-19.1932306152497", "module": "D", "scenario": "S3"}]}, "resolvedFlowVersion": "38.00.000", "flowProperties": [], "typeOfFlow": "Other flow", "classification": {"classHierarchy": "Quantities / Environmental quantities / EPD EN 15804 / LCI indicators", "name": "GaBiCategories"}}, {"dataSetInternalID": 7, "referenceToFlowDataSet": {"shortDescription": [{"value": "Use of secondary material (SM)", "lang": "en"}, {"value": "Einsatz von Sekundärstoffen (SM)", "lang": "de"}], "type": "flow data set", "refObjectId": "c6a1f35f-2d09-4f54-8dfb-97e502e1ce92", "uri": "../flows/c6a1f35f-2d09-4f54-8dfb-97e502e1ce92.xml"}, "exchange direction": "INPUT", "other": {"anies": [{"name": "referenceToUnitGroupDataSet", "value": {"shortDescription": [{"value": "kg", "lang": "en"}], "type": "unit group data set", "refObjectId": "ad38d542-3fe9-439d-9b95-2f5f7752acaf", "uri": "../unitgroups/ad38d542-3fe9-439d-9b95-2f5f7752acaf.xml"}}, {"value": "2.39", "module": "A1-A3"}, {"value": "0", "module": "A4"}, {"value": "0", "module": "A5"}, {"value": "0", "module": "C1"}, {"value": "0", "module": "C2"}, {"value": "0", "module": "C3", "scenario": "S1"}, {"value": "0", "module": "C3", "scenario": "S2"}, {"value": "0", "module": "C4"}, {"value": "0", "module": "D", "scenario": "S1"}, {"value": "30.4001879999999", "module": "D", "scenario": "S2"}, {"value": "0", "module": "D", "scenario": "S3"}]}, "resolvedFlowVersion": "38.00.000", "flowProperties": [], "typeOfFlow": "Other flow", "classification": {"classHierarchy": "Quantities / Environmental quantities / EPD EN 15804 / LCI indicators", "name": "GaBiCategories"}}, {"dataSetInternalID": 8, "referenceToFlowDataSet": {"shortDescription": [{"value": "Use of renewable secondary fuels (RSF)", "lang": "en"}, {"value": "Erneuerbare Sekundärbrennstoffe (RSF)", "lang": "de"}], "type": "flow data set", "refObjectId": "64333088-a55f-4aa2-9a31-c10b07816787", "uri": "../flows/64333088-a55f-4aa2-9a31-c10b07816787.xml"}, "exchange direction": "INPUT", "other": {"anies": [{"name": "referenceToUnitGroupDataSet", "value": {"shortDescription": [{"value": "MJ", "lang": "en"}], "type": "unit group data set", "refObjectId": "93a60a57-a3c8-11da-a746-0800200c9a66", "uri": "../unitgroups/93a60a57-a3c8-11da-a746-0800200c9a66.xml"}}, {"value": "0", "module": "A1-A3"}, {"value": "0", "module": "A4"}, {"value": "0", "module": "A5"}, {"value": "0", "module": "C1"}, {"value": "0", "module": "C2"}, {"value": "0", "module": "C3", "scenario": "S1"}, {"value": "0", "module": "C3", "scenario": "S2"}, {"value": "0", "module": "C4"}, {"value": "0", "module": "D", "scenario": "S1"}, {"value": "0", "module": "D", "scenario": "S2"}, {"value": "0", "module": "D", "scenario": "S3"}]}, "resolvedFlowVersion": "38.00.000", "flowProperties": [], "typeOfFlow": "Other flow", "classification": {"classHierarchy": "Quantities / Environmental quantities / EPD EN 15804 / LCI indicators", "name": "GaBiCategories"}}, {"dataSetInternalID": 9, "referenceToFlowDataSet": {"shortDescription": [{"value": "Use of non renewable secondary fuels (NRSF)", "lang": "en"}, {"value": "Nicht erneuerbare Sekundärbrennstoffe (NRSF)", "lang": "de"}], "type": "flow data set", "refObjectId": "89def144-d39a-4287-b86f-efde453ddcb2", "uri": "../flows/89def144-d39a-4287-b86f-efde453ddcb2.xml"}, "exchange direction": "INPUT", "other": {"anies": [{"name": "referenceToUnitGroupDataSet", "value": {"shortDescription": [{"value": "MJ", "lang": "en"}], "type": "unit group data set", "refObjectId": "93a60a57-a3c8-11da-a746-0800200c9a66", "uri": "../unitgroups/93a60a57-a3c8-11da-a746-0800200c9a66.xml"}}, {"value": "0", "module": "A1-A3"}, {"value": "0", "module": "A4"}, {"value": "0", "module": "A5"}, {"value": "0", "module": "C1"}, {"value": "0", "module": "C2"}, {"value": "0", "module": "C3", "scenario": "S1"}, {"value": "0", "module": "C3", "scenario": "S2"}, {"value": "0", "module": "C4"}, {"value": "0", "module": "D", "scenario": "S1"}, {"value": "0", "module": "D", "scenario": "S2"}, {"value": "0", "module": "D", "scenario": "S3"}]}, "resolvedFlowVersion": "38.00.000", "flowProperties": [], "typeOfFlow": "Other flow", "classification": {"classHierarchy": "Quantities / Environmental quantities / EPD EN 15804 / LCI indicators", "name": "GaBiCategories"}}, {"dataSetInternalID": 10, "referenceToFlowDataSet": {"shortDescription": [{"value": "Use of net fresh water (FW)", "lang": "en"}, {"value": "Einsatz von Süßwasserressourcen (FW)", "lang": "de"}], "type": "flow data set", "refObjectId": "3cf952c8-f3a4-461d-8c96-96456ca62246", "uri": "../flows/3cf952c8-f3a4-461d-8c96-96456ca62246.xml"}, "exchange direction": "INPUT", "other": {"anies": [{"name": "referenceToUnitGroupDataSet", "value": {"shortDescription": [{"value": "m^3", "lang": "en"}], "type": "unit group data set", "refObjectId": "cd950537-0a98-4044-9ba7-9f9a68d0a504", "uri": "../unitgroups/cd950537-0a98-4044-9ba7-9f9a68d0a504.xml"}}, {"value": "0.437049761097288", "module": "A1-A3"}, {"value": "0.0013625311601685", "module": "A4"}, {"value": "0.00432417480269014", "module": "A5"}, {"value": "0", "module": "C1"}, {"value": "0.000133720327731911", "module": "C2"}, {"value": "0.220052785775173", "module": "C3", "scenario": "S1"}, {"value": "0.0437059815316267", "module": "C3", "scenario": "S2"}, {"value": "0.000348105880631389", "module": "C4"}, {"value": "-0.118371695957926", "module": "D", "scenario": "S1"}, {"value": "-0.346105030764754", "module": "D", "scenario": "S2"}, {"value": "-0.00251853407162117", "module": "D", "scenario": "S3"}]}, "resolvedFlowVersion": "38.00.000", "flowProperties": [], "typeOfFlow": "Other flow", "classification": {"classHierarchy": "Quantities / Environmental quantities / EPD EN 15804 / LCI indicators", "name": "GaBiCategories"}}, {"dataSetInternalID": 11, "referenceToFlowDataSet": {"shortDescription": [{"value": "Hazardous waste disposed (HWD)", "lang": "en"}, {"value": "Gefährlicher Abfall zur Deponie (HWD)", "lang": "de"}], "type": "flow data set", "refObjectId": "430f9e0f-59b2-46a0-8e0d-55e0e84948fc", "uri": "../flows/430f9e0f-59b2-46a0-8e0d-55e0e84948fc.xml"}, "exchange direction": "OUTPUT", "other": {"anies": [{"name": "referenceToUnitGroupDataSet", "value": {"shortDescription": [{"value": "kg", "lang": "en"}], "type": "unit group data set", "refObjectId": "ad38d542-3fe9-439d-9b95-2f5f7752acaf", "uri": "../unitgroups/ad38d542-3fe9-439d-9b95-2f5f7752acaf.xml"}}, {"value": "1.7932845961748E-07", "module": "A1-A3"}, {"value": "5.31289550240173E-11", "module": "A4"}, {"value": "5.34735905557094E-12", "module": "A5"}, {"value": "0", "module": "C1"}, {"value": "5.21413490241705E-12", "module": "C2"}, {"value": "2.71250252137743E-10", "module": "C3", "scenario": "S1"}, {"value": "-7.08743419779558E-09", "module": "C3", "scenario": "S2"}, {"value": "2.97269562160918E-09", "module": "C4"}, {"value": "-9.89980363451442E-08", "module": "D", "scenario": "S1"}, {"value": "-1.08869466331273E-07", "module": "D", "scenario": "S2"}, {"value": "-2.10402872997171E-09", "module": "D", "scenario": "S3"}]}, "resolvedFlowVersion": "38.00.000", "flowProperties": [], "typeOfFlow": "Other flow", "classification": {"classHierarchy": "Quantities / Environmental quantities / EPD EN 15804 / LCI indicators", "name": "GaBiCategories"}}, {"dataSetInternalID": 12, "referenceToFlowDataSet": {"shortDescription": [{"value": "Non hazardous waste disposed (NHWD)", "lang": "en"}, {"value": "Entsorgter nicht gefährlicher Abfall (NHWD)", "lang": "de"}], "type": "flow data set", "refObjectId": "b29ef66b-e286-4afa-949f-62f1a7b4d7fa", "uri": "../flows/b29ef66b-e286-4afa-949f-62f1a7b4d7fa.xml"}, "exchange direction": "OUTPUT", "other": {"anies": [{"name": "referenceToUnitGroupDataSet", "value": {"shortDescription": [{"value": "kg", "lang": "en"}], "type": "unit group data set", "refObjectId": "ad38d542-3fe9-439d-9b95-2f5f7752acaf", "uri": "../unitgroups/ad38d542-3fe9-439d-9b95-2f5f7752acaf.xml"}}, {"value": "0.902684627675066", "module": "A1-A3"}, {"value": "0.00261566620375513", "module": "A4"}, {"value": "0.00956514566348914", "module": "A5"}, {"value": "0", "module": "C1"}, {"value": "0.000256704398569612", "module": "C2"}, {"value": "0.661718566749571", "module": "C3", "scenario": "S1"}, {"value": "0.0663377313695998", "module": "C3", "scenario": "S2"}, {"value": "34.2339417550734", "module": "C4"}, {"value": "-0.218241248644059", "module": "D", "scenario": "S1"}, {"value": "-0.550086467515228", "module": "D", "scenario": "S2"}, {"value": "-0.00463992755207981", "module": "D", "scenario": "S3"}]}, "resolvedFlowVersion": "38.00.000", "flowProperties": [], "typeOfFlow": "Other flow", "classification": {"classHierarchy": "Quantities / Environmental quantities / EPD EN 15804 / LCI indicators", "name": "GaBiCategories"}}, {"dataSetInternalID": 13, "referenceToFlowDataSet": {"shortDescription": [{"value": "Radioactive waste disposed (RWD)", "lang": "en"}, {"value": "Entsorgter radioaktiver Abfall (RWD)", "lang": "de"}], "type": "flow data set", "refObjectId": "3449546e-52ad-4b39-b809-9fb77cea8ff6", "uri": "../flows/3449546e-52ad-4b39-b809-9fb77cea8ff6.xml"}, "exchange direction": "OUTPUT", "other": {"anies": [{"name": "referenceToUnitGroupDataSet", "value": {"shortDescription": [{"value": "kg", "lang": "en"}], "type": "unit group data set", "refObjectId": "ad38d542-3fe9-439d-9b95-2f5f7752acaf", "uri": "../unitgroups/ad38d542-3fe9-439d-9b95-2f5f7752acaf.xml"}}, {"value": "0.0506416722719285", "module": "A1-A3"}, {"value": "3.21115919480801E-05", "module": "A4"}, {"value": "1.46615964706165E-05", "module": "A5"}, {"value": "0", "module": "C1"}, {"value": "3.15146744883217E-06", "module": "C2"}, {"value": "0.000781797982585197", "module": "C3", "scenario": "S1"}, {"value": "0.0143986682242557", "module": "C3", "scenario": "S2"}, {"value": "0.000417950055809986", "module": "C4"}, {"value": "-0.0795869461219001", "module": "D", "scenario": "S1"}, {"value": "-0.0131319374865299", "module": "D", "scenario": "S2"}, {"value": "-0.00169335920827122", "module": "D", "scenario": "S3"}]}, "resolvedFlowVersion": "38.00.000", "flowProperties": [], "typeOfFlow": "Other flow", "classification": {"classHierarchy": "Quantities / Environmental quantities / EPD EN 15804 / LCI indicators", "name": "GaBiCategories"}}, {"dataSetInternalID": 14, "referenceToFlowDataSet": {"shortDescription": [{"value": "Components for re-use (CRU)", "lang": "en"}, {"value": "Komponenten für die Wiederverwendung (CRU)", "lang": "de"}], "type": "flow data set", "refObjectId": "a2b32f97-3fc7-4af2-b209-525bc6426f33", "uri": "../flows/a2b32f97-3fc7-4af2-b209-525bc6426f33.xml"}, "exchange direction": "OUTPUT", "other": {"anies": [{"name": "referenceToUnitGroupDataSet", "value": {"shortDescription": [{"value": "kg", "lang": "en"}], "type": "unit group data set", "refObjectId": "ad38d542-3fe9-439d-9b95-2f5f7752acaf", "uri": "../unitgroups/ad38d542-3fe9-439d-9b95-2f5f7752acaf.xml"}}, {"value": "0", "module": "A1-A3"}, {"value": "0", "module": "A4"}, {"value": "0", "module": "A5"}, {"value": "0", "module": "C1"}, {"value": "0", "module": "C2"}, {"value": "0", "module": "C3", "scenario": "S1"}, {"value": "0", "module": "C3", "scenario": "S2"}, {"value": "0", "module": "C4"}, {"value": "0", "module": "D", "scenario": "S1"}, {"value": "0", "module": "D", "scenario": "S2"}, {"value": "0", "module": "D", "scenario": "S3"}]}, "resolvedFlowVersion": "38.00.000", "flowProperties": [], "typeOfFlow": "Other flow", "classification": {"classHierarchy": "Quantities / Environmental quantities / EPD EN 15804 / LCI indicators", "name": "GaBiCategories"}}, {"dataSetInternalID": 15, "referenceToFlowDataSet": {"shortDescription": [{"value": "Materials for recycling (MFR)", "lang": "en"}, {"value": "Stoffe zum Recycling (MFR)", "lang": "de"}], "type": "flow data set", "refObjectId": "d7fe48a5-4103-49c8-9aae-b0b5dfdbd6ae", "uri": "../flows/d7fe48a5-4103-49c8-9aae-b0b5dfdbd6ae.xml"}, "exchange direction": "OUTPUT", "other": {"anies": [{"name": "referenceToUnitGroupDataSet", "value": {"shortDescription": [{"value": "kg", "lang": "en"}], "type": "unit group data set", "refObjectId": "ad38d542-3fe9-439d-9b95-2f5f7752acaf", "uri": "../unitgroups/ad38d542-3fe9-439d-9b95-2f5f7752acaf.xml"}}, {"value": "0", "module": "A1-A3"}, {"value": "0", "module": "A4"}, {"value": "0", "module": "A5"}, {"value": "0", "module": "C1"}, {"value": "0", "module": "C2"}, {"value": "0", "module": "C3", "scenario": "S1"}, {"value": "34.37", "module": "C3", "scenario": "S2"}, {"value": "0", "module": "C4"}, {"value": "0", "module": "D", "scenario": "S1"}, {"value": "0", "module": "D", "scenario": "S2"}, {"value": "0", "module": "D", "scenario": "S3"}]}, "resolvedFlowVersion": "38.00.000", "flowProperties": [], "typeOfFlow": "Other flow", "classification": {"classHierarchy": "Quantities / Environmental quantities / EPD EN 15804 / LCI indicators", "name": "GaBiCategories"}}, {"dataSetInternalID": 16, "referenceToFlowDataSet": {"shortDescription": [{"value": "Materials for energy recovery (MER)", "lang": "en"}, {"value": "Stoffe für die Energierückgewinnung (MER)", "lang": "de"}], "type": "flow data set", "refObjectId": "59a9181c-3aaf-46ee-8b13-2b3723b6e447", "uri": "../flows/59a9181c-3aaf-46ee-8b13-2b3723b6e447.xml"}, "exchange direction": "OUTPUT", "other": {"anies": [{"name": "referenceToUnitGroupDataSet", "value": {"shortDescription": [{"value": "kg", "lang": "en"}], "type": "unit group data set", "refObjectId": "ad38d542-3fe9-439d-9b95-2f5f7752acaf", "uri": "../unitgroups/ad38d542-3fe9-439d-9b95-2f5f7752acaf.xml"}}, {"value": "0", "module": "A1-A3"}, {"value": "0", "module": "A4"}, {"value": "0", "module": "A5"}, {"value": "0", "module": "C1"}, {"value": "0", "module": "C2"}, {"value": "0", "module": "C3", "scenario": "S1"}, {"value": "0", "module": "C3", "scenario": "S2"}, {"value": "0", "module": "C4"}, {"value": "0", "module": "D", "scenario": "S1"}, {"value": "0", "module": "D", "scenario": "S2"}, {"value": "0", "module": "D", "scenario": "S3"}]}, "resolvedFlowVersion": "38.00.000", "flowProperties": [], "typeOfFlow": "Other flow", "classification": {"classHierarchy": "Quantities / Environmental quantities / EPD EN 15804 / LCI indicators", "name": "GaBiCategories"}}, {"dataSetInternalID": 17, "referenceToFlowDataSet": {"shortDescription": [{"value": "Exported electrical energy (EEE)", "lang": "en"}, {"value": "Exportierte elektrische Energie (EEE)", "lang": "de"}], "type": "flow data set", "refObjectId": "4da0c987-2b76-40d6-9e9e-82a017aaaf29", "uri": "../flows/4da0c987-2b76-40d6-9e9e-82a017aaaf29.xml"}, "exchange direction": "OUTPUT", "other": {"anies": [{"name": "referenceToUnitGroupDataSet", "value": {"shortDescription": [{"value": "MJ", "lang": "en"}], "type": "unit group data set", "refObjectId": "93a60a57-a3c8-11da-a746-0800200c9a66", "uri": "../unitgroups/93a60a57-a3c8-11da-a746-0800200c9a66.xml"}}, {"value": "0", "module": "A1-A3"}, {"value": "0", "module": "A4"}, {"value": "4.21534059931044", "module": "A5"}, {"value": "0", "module": "C1"}, {"value": "0", "module": "C2"}, {"value": "208.393995946892", "module": "C3", "scenario": "S1"}, {"value": "0", "module": "C3", "scenario": "S2"}, {"value": "0", "module": "C4"}, {"value": "0", "module": "D", "scenario": "S1"}, {"value": "0", "module": "D", "scenario": "S2"}, {"value": "0", "module": "D", "scenario": "S3"}]}, "resolvedFlowVersion": "38.00.000", "flowProperties": [], "typeOfFlow": "Other flow", "classification": {"classHierarchy": "Quantities / Environmental quantities / EPD EN 15804 / LCI indicators", "name": "GaBiCategories"}}, {"dataSetInternalID": 18, "referenceToFlowDataSet": {"shortDescription": [{"value": "Exported thermal energy (EET)", "lang": "en"}, {"value": "Exportierte thermische Energie (EET)", "lang": "de"}], "type": "flow data set", "refObjectId": "98daf38a-7a79-46d3-9a37-2b7bd0955810", "uri": "../flows/98daf38a-7a79-46d3-9a37-2b7bd0955810.xml"}, "exchange direction": "OUTPUT", "other": {"anies": [{"name": "referenceToUnitGroupDataSet", "value": {"shortDescription": [{"value": "MJ", "lang": "en"}], "type": "unit group data set", "refObjectId": "93a60a57-a3c8-11da-a746-0800200c9a66", "uri": "../unitgroups/93a60a57-a3c8-11da-a746-0800200c9a66.xml"}}, {"value": "0", "module": "A1-A3"}, {"value": "0", "module": "A4"}, {"value": "7.50097821512156", "module": "A5"}, {"value": "0", "module": "C1"}, {"value": "0", "module": "C2"}, {"value": "371.428005757475", "module": "C3", "scenario": "S1"}, {"value": "0", "module": "C3", "scenario": "S2"}, {"value": "0", "module": "C4"}, {"value": "0", "module": "D", "scenario": "S1"}, {"value": "0", "module": "D", "scenario": "S2"}, {"value": "0", "module": "D", "scenario": "S3"}]}, "resolvedFlowVersion": "38.00.000", "flowProperties": [], "typeOfFlow": "Other flow", "classification": {"classHierarchy": "Quantities / Environmental quantities / EPD EN 15804 / LCI indicators", "name": "GaBiCategories"}}]}, "LCIAResults": {"LCIAResult": [{"referenceToLCIAMethodDataSet": {"shortDescription": [{"value": "Global Warming Potential total (GWP-total)", "lang": "en"}, {"value": "Globales Erwärmungspotenzial total (GWP-total)", "lang": "de"}], "type": "LCIA method data set", "refObjectId": "6a37f984-a4b3-458a-a20a-64418c145fa2", "uri": "../lciamethods/6a37f984-a4b3-458a-a20a-64418c145fa2.xml"}, "other": {"anies": [{"name": "referenceToUnitGroupDataSet", "value": {"shortDescription": [{"value": "kg CO_(2) eq", "lang": "en"}], "type": "unit group data set", "refObjectId": "1ebf3012-d0db-4de2-aefd-ef30cedb0be1", "uri": "../unitgroups/1ebf3012-d0db-4de2-aefd-ef30cedb0be1.xml"}}, {"value": "103.818947607327", "module": "A1-A3"}, {"value": "1.2693975409142", "module": "A4"}, {"value": "2.08547778360084", "module": "A5"}, {"value": "0", "module": "C1"}, {"value": "0.124580090463496", "module": "C2"}, {"value": "115.088727313567", "module": "C3", "scenario": "S1"}, {"value": "4.40143955508202", "module": "C3", "scenario": "S2"}, {"value": "2.44113168562387", "module": "C4"}, {"value": "-47.2727618843682", "module": "D", "scenario": "S1"}, {"value": "-68.2599627676377", "module": "D", "scenario": "S2"}, {"value": "-1.005006733431", "module": "D", "scenario": "S3"}]}}, {"referenceToLCIAMethodDataSet": {"shortDescription": [{"value": "Global Warming Potential fossil fuels (GWP-fossil)", "lang": "en"}, {"value": "Globales Erwärmungspotenzial fossil (GWP-fossil)", "lang": "de"}], "type": "LCIA method data set", "refObjectId": "5f635281-343e-44fb-83df-1971b155e6b6", "uri": "../lciamethods/5f635281-343e-44fb-83df-1971b155e6b6.xml"}, "other": {"anies": [{"name": "referenceToUnitGroupDataSet", "value": {"shortDescription": [{"value": "kg CO_(2) eq", "lang": "en"}], "type": "unit group data set", "refObjectId": "1ebf3012-d0db-4de2-aefd-ef30cedb0be1", "uri": "../unitgroups/1ebf3012-d0db-4de2-aefd-ef30cedb0be1.xml"}}, {"value": "103.322387923614", "module": "A1-A3"}, {"value": "1.25764482582438", "module": "A4"}, {"value": "2.08540622423688", "module": "A5"}, {"value": "0", "module": "C1"}, {"value": "0.123426665896416", "module": "C2"}, {"value": "115.084935091967", "module": "C3", "scenario": "S1"}, {"value": "4.35377724191542", "module": "C3", "scenario": "S2"}, {"value": "2.43599734407922", "module": "C4"}, {"value": "-47.2140351000632", "module": "D", "scenario": "S1"}, {"value": "-67.9851688846853", "module": "D", "scenario": "S2"}, {"value": "-1.00375872929371", "module": "D", "scenario": "S3"}]}}, {"referenceToLCIAMethodDataSet": {"shortDescription": [{"value": "Global Warming Potential biogenic (GWP-biogenic)", "lang": "en"}, {"value": "Globales Erwärmungspotenzial biogen (GWP-biogenic)", "lang": "de"}], "type": "LCIA method data set", "refObjectId": "2356e1ab-0185-4db5-86e5-16de51c7485c", "uri": "../lciamethods/2356e1ab-0185-4db5-86e5-16de51c7485c.xml"}, "other": {"anies": [{"name": "referenceToUnitGroupDataSet", "value": {"shortDescription": [{"value": "kg CO_(2) eq", "lang": "en"}], "type": "unit group data set", "refObjectId": "1ebf3012-d0db-4de2-aefd-ef30cedb0be1", "uri": "../unitgroups/1ebf3012-d0db-4de2-aefd-ef30cedb0be1.xml"}}, {"value": "0.479491296328634", "module": "A1-A3"}, {"value": "0.000131067158194859", "module": "A4"}, {"value": "6.93472341783533E-05", "module": "A5"}, {"value": "0", "module": "C1"}, {"value": "1.28630770884833E-05", "module": "C2"}, {"value": "0.00365433189467468", "module": "C3", "scenario": "S1"}, {"value": "0.0471945774761446", "module": "C3", "scenario": "S2"}, {"value": "0.00318878359665362", "module": "C4"}, {"value": "-0.055818581764294", "module": "D", "scenario": "S1"}, {"value": "-0.27072780842266", "module": "D", "scenario": "S2"}, {"value": "-0.00118615307078887", "module": "D", "scenario": "S3"}]}}, {"referenceToLCIAMethodDataSet": {"shortDescription": [{"value": "Global Warming Potential luluc (GWP-luluc)", "lang": "en"}, {"value": "Globales Erwärmungspotenzial luluc (GWP-luluc)", "lang": "de"}], "type": "LCIA method data set", "refObjectId": "4331bbdb-978a-490d-8707-eeb047f01a55", "uri": "../lciamethods/4331bbdb-978a-490d-8707-eeb047f01a55.xml"}, "other": {"anies": [{"name": "referenceToUnitGroupDataSet", "value": {"shortDescription": [{"value": "kg CO_(2) eq", "lang": "en"}], "type": "unit group data set", "refObjectId": "1ebf3012-d0db-4de2-aefd-ef30cedb0be1", "uri": "../unitgroups/1ebf3012-d0db-4de2-aefd-ef30cedb0be1.xml"}}, {"value": "0.0170683873837063", "module": "A1-A3"}, {"value": "0.0116216479316192", "module": "A4"}, {"value": "2.21212978328435E-06", "module": "A5"}, {"value": "0", "module": "C1"}, {"value": "0.00114056148999101", "module": "C2"}, {"value": "0.000137889706006314", "module": "C3", "scenario": "S1"}, {"value": "0.00046773569045713", "module": "C3", "scenario": "S2"}, {"value": "0.00194555794799782", "module": "C4"}, {"value": "-0.00290820254071478", "module": "D", "scenario": "S1"}, {"value": "-0.00406607452977627", "module": "D", "scenario": "S2"}, {"value": "-6.18510665046123E-05", "module": "D", "scenario": "S3"}]}}, {"referenceToLCIAMethodDataSet": {"shortDescription": [{"value": "Depletion potential of the stratospheric ozone layer (ODP)", "lang": "en"}, {"value": "Abbau Potential der stratosphärischen Ozonschicht (ODP)", "lang": "de"}], "type": "LCIA method data set", "refObjectId": "b5c629d6-def3-11e6-bf01-fe55135034f3", "uri": "../lciamethods/b5c629d6-def3-11e6-bf01-fe55135034f3.xml"}, "other": {"anies": [{"name": "referenceToUnitGroupDataSet", "value": {"shortDescription": [{"value": "kg CFC11 eq", "lang": "en"}], "type": "unit group data set", "refObjectId": "d9e957c9-7309-4474-bf3a-7777df6c4e5b", "uri": "../unitgroups/d9e957c9-7309-4474-bf3a-7777df6c4e5b.xml"}}, {"value": "1.41985166386688E-10", "module": "A1-A3"}, {"value": "1.63276374816016E-13", "module": "A4"}, {"value": "9.78705444582588E-14", "module": "A5"}, {"value": "0", "module": "C1"}, {"value": "1.60241255316138E-14", "module": "C2"}, {"value": "5.31638000519057E-12", "module": "C3", "scenario": "S1"}, {"value": "7.94049190366292E-11", "module": "C3", "scenario": "S2"}, {"value": "3.97209778204533E-12", "module": "C4"}, {"value": "-2.29303436851448E-10", "module": "D", "scenario": "S1"}, {"value": "-6.9456690476889E-11", "module": "D", "scenario": "S2"}, {"value": "-4.87883342675643E-12", "module": "D", "scenario": "S3"}]}}, {"referenceToLCIAMethodDataSet": {"shortDescription": [{"value": "Acidification potential of land and water (AP)", "lang": "en"}, {"value": "Versauerungspotenzial von Boden und Wasser (AP)", "lang": "de"}], "type": "LCIA method data set", "refObjectId": "b5c611c6-def3-11e6-bf01-fe55135034f3", "uri": "../lciamethods/b5c611c6-def3-11e6-bf01-fe55135034f3.xml"}, "other": {"anies": [{"name": "referenceToUnitGroupDataSet", "value": {"shortDescription": [{"value": "mol H^(+) eq", "lang": "en"}], "type": "unit group data set", "refObjectId": "42e089ac-92bf-4bf2-8ca1-5fc40d18f2ed", "uri": "../unitgroups/42e089ac-92bf-4bf2-8ca1-5fc40d18f2ed.xml"}}, {"value": "0.143714414189785", "module": "A1-A3"}, {"value": "0.00161034204928006", "module": "A4"}, {"value": "0.000197463100000232", "module": "A5"}, {"value": "0", "module": "C1"}, {"value": "0.000158040764780433", "module": "C2"}, {"value": "0.0100523673131026", "module": "C3", "scenario": "S1"}, {"value": "0.00919084181220939", "module": "C3", "scenario": "S2"}, {"value": "0.00709047970911372", "module": "C4"}, {"value": "-0.0495315928310621", "module": "D", "scenario": "S1"}, {"value": "-0.105514821778696", "module": "D", "scenario": "S2"}, {"value": "-0.0010534006666846", "module": "D", "scenario": "S3"}]}}, {"referenceToLCIAMethodDataSet": {"shortDescription": [{"value": "Eutrophication potential aquatic freshwater (EP-freshwater)", "lang": "en"}, {"value": "Eutrophierungspotenzial Süßwasser (EP-freshwater)", "lang": "de"}], "type": "LCIA method data set", "refObjectId": "b53ec18f-7377-4ad3-86eb-cc3f4f276b2b", "uri": "../lciamethods/b53ec18f-7377-4ad3-86eb-cc3f4f276b2b.xml"}, "other": {"anies": [{"name": "referenceToUnitGroupDataSet", "value": {"shortDescription": [{"value": "kg P eq", "lang": "en"}], "type": "unit group data set", "refObjectId": "0429039d-a61d-4590-ba67-aa4a20a810a1", "uri": "../unitgroups/0429039d-a61d-4590-ba67-aa4a20a810a1.xml"}}, {"value": "0.000112521401411675", "module": "A1-A3"}, {"value": "4.58784078110845E-06", "module": "A4"}, {"value": "2.32663135677533E-08", "module": "A5"}, {"value": "0", "module": "C1"}, {"value": "4.50255811218119E-07", "module": "C2"}, {"value": "1.2694431570287E-06", "module": "C3", "scenario": "S1"}, {"value": "1.60538834958513E-05", "module": "C3", "scenario": "S2"}, {"value": "0.000454960000804895", "module": "C4"}, {"value": "-2.44846467228385E-05", "module": "D", "scenario": "S1"}, {"value": "-8.0549827457693E-05", "module": "D", "scenario": "S2"}, {"value": "-5.20905689681297E-07", "module": "D", "scenario": "S3"}]}}, {"referenceToLCIAMethodDataSet": {"shortDescription": [{"value": "Eutrophication potential aquatic marine (EP-marine)", "lang": "en"}, {"value": "Eutrophierungspotenzial Salzwasser (EP-marine)", "lang": "de"}], "type": "LCIA method data set", "refObjectId": "b5c619fa-def3-11e6-bf01-fe55135034f3", "uri": "../lciamethods/b5c619fa-def3-11e6-bf01-fe55135034f3.xml"}, "other": {"anies": [{"name": "referenceToUnitGroupDataSet", "value": {"shortDescription": [{"value": "kg N eq", "lang": "en"}], "type": "unit group data set", "refObjectId": "d05bb823-ecdf-4686-8c40-bf1d9257859f", "uri": "../unitgroups/d05bb823-ecdf-4686-8c40-bf1d9257859f.xml"}}, {"value": "0.0418880228202065", "module": "A1-A3"}, {"value": "0.000545910498934488", "module": "A4"}, {"value": "4.20614298421166E-05", "module": "A5"}, {"value": "0", "module": "C1"}, {"value": "5.3576265236225E-05", "module": "C2"}, {"value": "0.00221564792456647", "module": "C3", "scenario": "S1"}, {"value": "0.00219896072476448", "module": "C3", "scenario": "S2"}, {"value": "0.00162432744010992", "module": "C4"}, {"value": "-0.0161005457436582", "module": "D", "scenario": "S1"}, {"value": "-0.0292060087315423", "module": "D", "scenario": "S2"}, {"value": "-0.000342362867245129", "module": "D", "scenario": "S3"}]}}, {"referenceToLCIAMethodDataSet": {"shortDescription": [{"value": "Eutrophication potential terrestrial (EP-terrestrial)", "lang": "en"}, {"value": "Eutrophierungspotenzial Land (EP-terrestrial)", "lang": "de"}], "type": "LCIA method data set", "refObjectId": "b5c614d2-def3-11e6-bf01-fe55135034f3", "uri": "../lciamethods/b5c614d2-def3-11e6-bf01-fe55135034f3.xml"}, "other": {"anies": [{"name": "referenceToUnitGroupDataSet", "value": {"shortDescription": [{"value": "mol N eq", "lang": "en"}], "type": "unit group data set", "refObjectId": "71b4d617-0ec9-4d3f-b65e-e438940c2401", "uri": "../unitgroups/71b4d617-0ec9-4d3f-b65e-e438940c2401.xml"}}, {"value": "0.457842171584769", "module": "A1-A3"}, {"value": "0.00656726965997186", "module": "A4"}, {"value": "0.000931099454526856", "module": "A5"}, {"value": "0", "module": "C1"}, {"value": "0.000644519169107772", "module": "C2"}, {"value": "0.0474633002425392", "module": "C3", "scenario": "S1"}, {"value": "0.0229767767372374", "module": "C3", "scenario": "S2"}, {"value": "0.0178355059829564", "module": "C4"}, {"value": "-0.173256705826739", "module": "D", "scenario": "S1"}, {"value": "-0.316133954198229", "module": "D", "scenario": "S2"}, {"value": "-0.00368407339740201", "module": "D", "scenario": "S3"}]}}, {"referenceToLCIAMethodDataSet": {"shortDescription": [{"value": "Formation potential of tropospheric ozone photochemical oxidants (POCP)", "lang": "en"}, {"value": "Bildungspotential für troposphärisches Ozon (POCP)", "lang": "de"}], "type": "LCIA method data set", "refObjectId": "b5c610fe-def3-11e6-bf01-fe55135034f3", "uri": "../lciamethods/b5c610fe-def3-11e6-bf01-fe55135034f3.xml"}, "other": {"anies": [{"name": "referenceToUnitGroupDataSet", "value": {"shortDescription": [{"value": "kg NMVOC eq", "lang": "en"}], "type": "unit group data set", "refObjectId": "d27c25f8-fbc1-44c6-b47b-4adbae4199c6", "uri": "../unitgroups/d27c25f8-fbc1-44c6-b47b-4adbae4199c6.xml"}}, {"value": "0.284192997509802", "module": "A1-A3"}, {"value": "0.00138822509338447", "module": "A4"}, {"value": "0.000124705972771087", "module": "A5"}, {"value": "0", "module": "C1"}, {"value": "0.000136241958994958", "module": "C2"}, {"value": "0.00652292050625518", "module": "C3", "scenario": "S1"}, {"value": "0.00586644890238308", "module": "C3", "scenario": "S2"}, {"value": "0.00515910125749475", "module": "C4"}, {"value": "-0.0456919718469732", "module": "D", "scenario": "S1"}, {"value": "-0.114026644520925", "module": "D", "scenario": "S2"}, {"value": "-0.000971571610870027", "module": "D", "scenario": "S3"}]}}, {"referenceToLCIAMethodDataSet": {"shortDescription": [{"value": "Abiotic depletion potential for non fossil resources (ADPE)", "lang": "en"}, {"value": "Potenzial für den abiotischen Abbau nicht fossiler Ressourcen (ADPE)", "lang": "de"}], "type": "LCIA method data set", "refObjectId": "b2ad6494-c78d-11e6-9d9d-cec0c932ce01", "uri": "../lciamethods/b2ad6494-c78d-11e6-9d9d-cec0c932ce01.xml"}, "other": {"anies": [{"name": "referenceToUnitGroupDataSet", "value": {"shortDescription": [{"value": "kg Sb eq", "lang": "en"}], "type": "unit group data set", "refObjectId": "54ccd2d9-a32a-4fc2-923d-f2c8c93e89d4", "uri": "../unitgroups/54ccd2d9-a32a-4fc2-923d-f2c8c93e89d4.xml"}}, {"value": "3.44243240468649E-05", "module": "A1-A3"}, {"value": "8.26408982586171E-08", "module": "A4"}, {"value": "9.1048634727992E-10", "module": "A5"}, {"value": "0", "module": "C1"}, {"value": "8.11046992703998E-09", "module": "C2"}, {"value": "4.93086138385277E-08", "module": "C3", "scenario": "S1"}, {"value": "6.67125153294429E-07", "module": "C3", "scenario": "S2"}, {"value": "6.24635601074546E-08", "module": "C4"}, {"value": "-1.37771195584317E-06", "module": "D", "scenario": "S1"}, {"value": "-2.04380317724489E-06", "module": "D", "scenario": "S2"}, {"value": "-2.93048962616966E-08", "module": "D", "scenario": "S3"}]}}, {"referenceToLCIAMethodDataSet": {"shortDescription": [{"value": "Abiotic depletion potential for fossil resources (ADPF)", "lang": "en"}, {"value": "Potenzial für den abiotischen Abbau fossiler Brennstoffe (ADPF)", "lang": "de"}], "type": "LCIA method data set", "refObjectId": "b2ad6110-c78d-11e6-9d9d-cec0c932ce01", "uri": "../lciamethods/b2ad6110-c78d-11e6-9d9d-cec0c932ce01.xml"}, "other": {"anies": [{"name": "referenceToUnitGroupDataSet", "value": {"shortDescription": [{"value": "MJ", "lang": "en"}], "type": "unit group data set", "refObjectId": "93a60a57-a3c8-11da-a746-0800200c9a66", "uri": "../unitgroups/93a60a57-a3c8-11da-a746-0800200c9a66.xml"}}, {"value": "2790.13168106204", "module": "A1-A3"}, {"value": "17.0940839240176", "module": "A4"}, {"value": "0.243676221498276", "module": "A5"}, {"value": "0", "module": "C1"}, {"value": "1.67763246186141", "module": "C2"}, {"value": "13.0174710212351", "module": "C3", "scenario": "S1"}, {"value": "90.5593789891434", "module": "C3", "scenario": "S2"}, {"value": "35.2826676263831", "module": "C4"}, {"value": "-902.58870495788", "module": "D", "scenario": "S1"}, {"value": "-2253.2806380165", "module": "D", "scenario": "S2"}, {"value": "-19.1910438630415", "module": "D", "scenario": "S3"}]}}, {"referenceToLCIAMethodDataSet": {"shortDescription": [{"value": "Water use (WDP)", "lang": "en"}, {"value": "Wassernutzung (WDP)", "lang": "de"}], "type": "LCIA method data set", "refObjectId": "b2ad66ce-c78d-11e6-9d9d-cec0c932ce01", "uri": "../lciamethods/b2ad66ce-c78d-11e6-9d9d-cec0c932ce01.xml"}, "other": {"anies": [{"name": "referenceToUnitGroupDataSet", "value": {"shortDescription": [{"value": "m^(3) world eq deprived", "lang": "en"}], "type": "unit group data set", "refObjectId": "6ae2df01-888e-46c8-b17d-49fa3869b476", "uri": "../unitgroups/6ae2df01-888e-46c8-b17d-49fa3869b476.xml"}}, {"value": "4.97270954975025", "module": "A1-A3"}, {"value": "0.01516321178443", "module": "A4"}, {"value": "0.18459303375166", "module": "A5"}, {"value": "0", "module": "C1"}, {"value": "0.00148813451652111", "module": "C2"}, {"value": "9.39054795356513", "module": "C3", "scenario": "S1"}, {"value": "0.95897813123193", "module": "C3", "scenario": "S2"}, {"value": "-0.0333665071393359", "module": "C4"}, {"value": "-1.9755294623703", "module": "D", "scenario": "S1"}, {"value": "-13.9355425125355", "module": "D", "scenario": "S2"}, {"value": "-0.04203232216513", "module": "D", "scenario": "S3"}]}}, {"referenceToLCIAMethodDataSet": {"shortDescription": [{"value": "Incidence of disease due to PM emissions (PM)", "lang": "en"}, {"value": "Auftreten von Krankheiten aufgrund von Feinstaubemissionen (PM)", "lang": "de"}], "type": "LCIA method data set", "refObjectId": "b5c602c6-def3-11e6-bf01-fe55135034f3", "uri": "../lciamethods/b5c602c6-def3-11e6-bf01-fe55135034f3.xml"}, "other": {"anies": [{"name": "referenceToUnitGroupDataSet", "value": {"shortDescription": [{"value": "Disease incidence", "lang": "en"}], "type": "unit group data set", "refObjectId": "3883559b-648f-4afc-8ba2-0bd24f3affa3", "uri": "../unitgroups/3883559b-648f-4afc-8ba2-0bd24f3affa3.xml"}}, {"value": "1.1100386383939E-06", "module": "A1-A3"}, {"value": "1.17841222790483E-08", "module": "A4"}, {"value": "1.15608199615165E-09", "module": "A5"}, {"value": "0", "module": "C1"}, {"value": "1.15650690366034E-09", "module": "C2"}, {"value": "5.87187448774142E-08", "module": "C3", "scenario": "S1"}, {"value": "7.73631202776874E-08", "module": "C3", "scenario": "S2"}, {"value": "6.87319777800865E-08", "module": "C4"}, {"value": "-4.42457142110749E-07", "module": "D", "scenario": "S1"}, {"value": "-7.19901255884507E-07", "module": "D", "scenario": "S2"}, {"value": "-9.40997475027888E-09", "module": "D", "scenario": "S3"}]}}, {"referenceToLCIAMethodDataSet": {"shortDescription": [{"value": "Human exposure efficiency relative to U235 (IR)", "lang": "en"}, {"value": "Wirkung durch Exposition des Menschen mit U235 (IR)", "lang": "de"}], "type": "LCIA method data set", "refObjectId": "b5c632be-def3-11e6-bf01-fe55135034f3", "uri": "../lciamethods/b5c632be-def3-11e6-bf01-fe55135034f3.xml"}, "other": {"anies": [{"name": "referenceToUnitGroupDataSet", "value": {"shortDescription": [{"value": "kBq U235 eq", "lang": "en"}], "type": "unit group data set", "refObjectId": "456b05bf-1415-44a9-9993-02452f554c09", "uri": "../unitgroups/456b05bf-1415-44a9-9993-02452f554c09.xml"}}, {"value": "4.40836332714909", "module": "A1-A3"}, {"value": "0.00478867298809937", "module": "A4"}, {"value": "0.00236425798463873", "module": "A5"}, {"value": "0", "module": "C1"}, {"value": "0.000469965708006554", "module": "C2"}, {"value": "0.125655799516465", "module": "C3", "scenario": "S1"}, {"value": "2.39615801553137", "module": "C3", "scenario": "S2"}, {"value": "0.0618028738710814", "module": "C4"}, {"value": "-11.9479785242108", "module": "D", "scenario": "S1"}, {"value": "-2.0974451740512", "module": "D", "scenario": "S2"}, {"value": "-0.254215369606055", "module": "D", "scenario": "S3"}]}}, {"referenceToLCIAMethodDataSet": {"shortDescription": [{"value": "Comparative toxic unit for ecosystems (ETP-fw)", "lang": "en"}, {"value": "Toxizitätsvergleichseinheit für Ökosysteme (ETP-fw)", "lang": "de"}], "type": "LCIA method data set", "refObjectId": "ee1082d1-b0f7-43ca-a1f0-21e2a4a74511", "uri": "../lciamethods/ee1082d1-b0f7-43ca-a1f0-21e2a4a74511.xml"}, "other": {"anies": [{"name": "referenceToUnitGroupDataSet", "value": {"shortDescription": [{"value": "CTUe", "lang": "en"}], "type": "unit group data set", "refObjectId": "aa959ded-f1eb-4efb-9c5c-2d60be36b3e6", "uri": "../unitgroups/aa959ded-f1eb-4efb-9c5c-2d60be36b3e6.xml"}}, {"value": "1476.91810040285", "module": "A1-A3"}, {"value": "12.1411674545638", "module": "A4"}, {"value": "0.114348337872754", "module": "A5"}, {"value": "0", "module": "C1"}, {"value": "1.19154771540892", "module": "C2"}, {"value": "6.34305713825502", "module": "C3", "scenario": "S1"}, {"value": "39.937368817995", "module": "C3", "scenario": "S2"}, {"value": "33.5892702701054", "module": "C4"}, {"value": "-150.001519050086", "module": "D", "scenario": "S1"}, {"value": "-1297.87151786415", "module": "D", "scenario": "S2"}, {"value": "-3.19143477538035", "module": "D", "scenario": "S3"}]}}, {"referenceToLCIAMethodDataSet": {"shortDescription": [{"value": "Comparative toxic unit for humans (carcinogenic) (HTP-c)", "lang": "en"}, {"value": "Toxizitätsvergleichseinheit für Menschen (krebserregend) (HTP-c)", "lang": "de"}], "type": "LCIA method data set", "refObjectId": "2299222a-bbd8-474f-9d4f-4dd1f18aea7c", "uri": "../lciamethods/2299222a-bbd8-474f-9d4f-4dd1f18aea7c.xml"}, "other": {"anies": [{"name": "referenceToUnitGroupDataSet", "value": {"shortDescription": [{"value": "CTUh", "lang": "en"}], "type": "unit group data set", "refObjectId": "d4c9523e-2d7e-49fd-8469-998f547d3a70", "uri": "../unitgroups/d4c9523e-2d7e-49fd-8469-998f547d3a70.xml"}}, {"value": "2.86603329968111E-08", "module": "A1-A3"}, {"value": "2.48440378752494E-10", "module": "A4"}, {"value": "1.29061509573394E-11", "module": "A5"}, {"value": "0", "module": "C1"}, {"value": "2.43822158639766E-11", "module": "C2"}, {"value": "6.45565159482665E-10", "module": "C3", "scenario": "S1"}, {"value": "1.33249874141173E-09", "module": "C3", "scenario": "S2"}, {"value": "1.54577448013735E-09", "module": "C4"}, {"value": "-5.63826932944047E-09", "module": "D", "scenario": "S1"}, {"value": "-2.64305369043715E-08", "module": "D", "scenario": "S2"}, {"value": "-1.19863579816116E-10", "module": "D", "scenario": "S3"}]}}, {"referenceToLCIAMethodDataSet": {"shortDescription": [{"value": "Comparative toxic unit for humans (noncarcinogenic) (HTP-nc)", "lang": "en"}, {"value": "Toxizitätsvergleichseinheit für Menschen (nicht krebserregend) (HTP-nc)", "lang": "de"}], "type": "LCIA method data set", "refObjectId": "3af763a5-b7a1-48c9-9cee-1f223481fcef", "uri": "../lciamethods/3af763a5-b7a1-48c9-9cee-1f223481fcef.xml"}, "other": {"anies": [{"name": "referenceToUnitGroupDataSet", "value": {"shortDescription": [{"value": "CTUh", "lang": "en"}], "type": "unit group data set", "refObjectId": "d4c9523e-2d7e-49fd-8469-998f547d3a70", "uri": "../unitgroups/d4c9523e-2d7e-49fd-8469-998f547d3a70.xml"}}, {"value": "1.28744020749154E-06", "module": "A1-A3"}, {"value": "1.32244547968574E-08", "module": "A4"}, {"value": "3.89456375344088E-10", "module": "A5"}, {"value": "0", "module": "C1"}, {"value": "1.29786274340535E-09", "module": "C2"}, {"value": "1.99923988531416E-08", "module": "C3", "scenario": "S1"}, {"value": "3.2767059609516E-08", "module": "C3", "scenario": "S2"}, {"value": "1.2853960598781E-07", "module": "C4"}, {"value": "-2.63578353605726E-07", "module": "D", "scenario": "S1"}, {"value": "-1.06541784890434E-06", "module": "D", "scenario": "S2"}, {"value": "-5.60378886567926E-09", "module": "D", "scenario": "S3"}]}}, {"referenceToLCIAMethodDataSet": {"shortDescription": [{"value": "Soil quality index (SQP)", "lang": "en"}, {"value": "Bodenqualitätsindex (SQP)", "lang": "de"}], "type": "LCIA method data set", "refObjectId": "b2ad6890-c78d-11e6-9d9d-cec0c932ce01", "uri": "../lciamethods/b2ad6890-c78d-11e6-9d9d-cec0c932ce01.xml"}, "other": {"anies": [{"name": "referenceToUnitGroupDataSet", "value": {"shortDescription": [{"value": "SQP", "lang": "en"}], "type": "unit group data set", "refObjectId": "f130951c-e67f-4f7f-8dd4-665de3974e18", "uri": "../unitgroups/f130951c-e67f-4f7f-8dd4-665de3974e18.xml"}}, {"value": "61.7627629110679", "module": "A1-A3"}, {"value": "7.14259648944679", "module": "A4"}, {"value": "0.0769887777719729", "module": "A5"}, {"value": "0", "module": "C1"}, {"value": "0.700982385832172", "module": "C2"}, {"value": "4.13112739966407", "module": "C3", "scenario": "S1"}, {"value": "35.5394030107398", "module": "C3", "scenario": "S2"}, {"value": "3.05591697192922", "module": "C4"}, {"value": "-69.8952712874056", "module": "D", "scenario": "S1"}, {"value": "-32.2128380425835", "module": "D", "scenario": "S2"}, {"value": "-1.48712470591004", "module": "D", "scenario": "S3"}]}}]}, "otherAttributes": {"{http://www.indata.network/EPD/2019}epd-version": "1.2"}, "version": "1.1", "locations": "../ILCDLocations.xml"}