{"processInformation": {"dataSetInformation": {"UUID": "d5f9f2a2-7f99-4930-980c-73e0734592b0", "name": {"baseName": [{"value": "Sika® ViscoCrete®-6720", "lang": "en"}, {"value": "Sika® ViscoCrete®-6720", "lang": "de"}], "functionalUnitFlowProperties": [{"lang": "en"}]}, "classificationInformation": {"classification": [{"class": [{"value": "Mineralische Baustoffe", "level": 0, "classId": "1"}, {"value": "Mörtel und Beton", "level": 1, "classId": "1.4"}, {"value": "Betonzusatzmittel", "level": 2, "classId": "1.4.06"}], "name": "OEKOBAU.DAT"}, {"class": [{"value": "01 Basic materials and precursors", "level": 0}, {"value": "Products related to concrete, mortar and grout", "level": 1}, {"value": "Concrete admixtures", "level": 2}], "name": "IBUCategories"}]}, "generalComment": [{"value": "Sika® ViscoCrete®-6720 is a superplasticizing admixture for concrete that provides a strong water reduction and reduced mixing time. \n\nAdmixtures are liquid or powdery agents that are introduced in small amounts (<5% by mass of the cement content) to concrete while it is being mixed and that enhance the properties of the fresh and/or hardened concrete. \n\nPlasticizers and superplasticizers are admixtures which reduce the water content of mixed concrete without detriment to its consistency or enhance its slump with or without change to the water content or cause both effects simultaneously. They can also display a retarding effect when used as combination products. \n\nThe product needs a declaration of performance taking into consideration EN 934-2:2009+A1:2012, Admixtures for concrete, mortar and grout– Part 2: Concrete admixtures – Definitions, requirements, conformity, marking and labelling and the CE-marking.", "lang": "en"}, {"value": "Sika® ViscoCrete®-6720 ist ein superplastifizierendes Zusatzmittel der dritten Generation für Beton, das eine starke Wasserreduzierung und eine verkürzte Mischzeit ermöglicht. \n\nZusatzmittel sind flüssige oder pulverförmige Wirkstoffe, die in kleinen Mengen (< 5 Massenprozent des Zementgehalts) während des Mischens in den Beton eingebracht werden und die die Eigenschaften des frischen und/oder festen Betons verbessern. \nVerflüssiger und Fließmittel sind Zusatzstoffe, die den Wassergehalt des gemischten Betons ohne Beeinträchtigung seiner Konsistenz verringern oder sein Setzmaß mit oder ohne Veränderung des Wassergehalts erhöhen oder beide Effekte gleichzeitig bewirken. Sie können auch eine verzögernde Wirkung haben, wenn sie als Kombinationsprodukte verwendet werden. \n\nDas Produkt benötigt eine Leistungserklärung unter Berücksichtigung von EN 934-2:2009+A1:2012, Zusatzmittel für Beton, Mörtel und Einpressmörtel - Teil 2: Betonzusatzmittel - Definitionen, Anforderungen, Konformität, Kennzeichnung und Beschriftung sowie die CE-Kennzeichnung.", "lang": "de"}]}, "quantitativeReference": {"referenceToReferenceFlow": [0]}, "time": {"referenceYear": 2025, "dataSetValidUntil": 2030, "other": {"anies": [{"name": "publicationDateOfEPD", "value": 1737504000000}]}}, "geography": {"locationOfOperationSupplyOrProduction": {"location": "SE"}}, "technology": {"technologyDescriptionAndIncludedProcesses": [{"value": "Sika® ViscoCrete®-6720 is a third-generation super plasticizing additive for concrete that provides a strong water reduction and reduced mixing time. Plasticizers and superplasticizers are admixtures which reduce the water content of mixed concrete without detriment to its consistency or enhance its slump with or without change to the water content or cause both effects simultaneously. They can also display a retarding effect when used as combination products. The typical dosage of superplasticizers lies between 0.4 and 2.0% by mass in relation to the cement weight. Recommended dosage of Sika® ViscoCrete®-6720 is 0.15–1.50 % of cement weight. \nTechnical data: \nPlasticizers and superplasticizers must comply with the general requirements of EN 934-1:2008 and the additional requirements of EN 934-2:2009+A1:2012. \nThe corresponding requirements in line with EN 934-1:2008 and EN 934-2:2009+A1:2012 must be maintained. \nDeclared unit: \nThe EPD refers to the declared unit of 1kg of concrete admixture (Superplasticizer for concrete) applied into the building with a density of 1.03 g/ml in accordance with IBU PCR 04- 2023 part B.\nThe typical dosage of superplasticizers lies between 0.4 and 2.0% by mass in relation to the cement weight.\nRecommended dosage of Sika® ViscoCrete®-6720 is 0.15–1.50 % of cement weight.", "lang": "en"}, {"value": "Sika® ViscoCrete®-6720 ist ein Superplastifiziermittel der dritten Generation für Beton, das eine starke Wasserreduzierung und eine verkürzte Mischzeit ermöglicht.\n\nPlastifiziermittel und Superplastifizierer sind Zusatzmittel, die den Wassergehalt von gemischtem Beton ohne Beeinträchtigung seiner Konsistenz reduzieren oder sein Absacken mit oder ohne Änderung des Wassergehalts verbessern oder beide Effekte gleichzeitig bewirken. Sie können auch eine verzögernde Wirkung haben, wenn sie als Kombinationsprodukte verwendet werden.\n\nDie typische Dosierung von Superplastifizierern liegt zwischen 0,4 und 2,0 Massen-% im Verhältnis zum Zementgewicht. Die empfohlene Dosierung von Sika® ViscoCrete®-6720 beträgt 0,15–1,50 % des Zementgewichts. \nTechnische Daten: \nWeichmacher und Fließmittel müssen den allgemeinen Anforderungen der EN 934-1:2008 und den zusätzlichen Anforderungen der EN 934-2:2009+A1:2012 entsprechen. \nDie entsprechenden Anforderungen gemäß EN 934-1:2008 und EN 934-2:2009+A1:2012 müssen eingehalten werden. \nDeklarierte Einheit: \nDie EPD bezieht sich auf die deklarierte Einheit von 1 kg Betonzusatzmittel (Fließmittel für Beton), das mit einer Dichte von 1,03 g/ml gemäß IBU PCR 04- 2023 Teil B in das Gebäude eingebracht wird. Die typische Dosierung von Fließmitteln liegt zwischen 0,4 und 2,0 Massenprozent im Verhältnis zum Zementgewicht. Die empfohlene Dosierung von Sika® ViscoCrete®-6720 liegt bei 0,15-1,50 % des Zementgewichts.", "lang": "de"}], "technologicalApplicability": [{"value": "Sika® ViscoCrete®-6720 is particularly suitable for the production of concrete mixes that require powerful water reduction and excellent flowability.\n\n▪ Concrete with low water content\n▪ Self-compacting concrete \n▪ Crushed aggregate \n▪ Concrete with high strength\n\nSika® ViscoCrete®-6720 provides good dispersing properties, resulting in a short mixing time.\n▪ Short mixing time \n▪ Shorter production times \n▪ Excellent workability \n▪ Developed for blended cement \n▪ Control over poor quality aggregate \n▪ Good strength development \n▪ Improved rheology \n▪ Excellent pumpability, viscosity lowering \n▪ Less labor-intensive when laying out and compacting", "lang": "en"}, {"value": "Sika® ViscoCrete®-6720 eignet sich besonders für die Herstellung von Betonmischungen, die eine starke Wasserreduzierung und eine hervorragende Fließfähigkeit erfordern. ▪ Beton mit niedrigem Wassergehalt ▪ Selbstverdichtender Beton ▪ Zerkleinerte Zuschlagstoffe ▪ Beton mit hoher Festigkeit Sika® ViscoCrete®-6720 bietet gute Dispergiereigenschaften, was zu einer kurzen Mischzeit führt.\n▪ Kurze Mischzeit ▪ Kürzere Produktionszeiten ▪ Hervorragende Verarbeitbarkeit ▪ Entwickelt für gemischten Zement ▪ Kontrolle über minderwertige Zuschlagstoffe ▪ Gute Festigkeitsentwicklung ▪ Verbesserte Rheologie ▪ Hervorragende Pumpfähigkeit, Viskositätssenkung ▪ Weniger arbeitsintensiv beim Auslegen und Verdichten", "lang": "de"}]}}, "modellingAndValidation": {"LCIMethodAndAllocation": {"typeOfDataSet": "EPD", "referenceToLCAMethodDetails": [{"shortDescription": [{"value": "Concrete admixtures.pdf", "lang": "en"}], "type": "source data set", "refObjectId": "126e45ff-fb38-488c-89bc-abab5998ad7e"}], "other": {"anies": [{"name": "subType", "value": "specific dataset"}]}}, "dataSourcesTreatmentAndRepresentativeness": {"referenceToDataSource": [{"shortDescription": [{"value": "GaBi Database (all versions)", "lang": "en"}], "type": "source data set", "refObjectId": "28d74cc0-db8b-4d7e-bc44-5f6d56ce0c4a"}, {"shortDescription": [{"value": "Sphera MLC (fka GaBi) Databases Edition 2024", "lang": "en"}], "type": "source data set", "refObjectId": "7443b962-0446-4d69-8aa7-8055a6b1614a"}], "useAdviceForDataSet": [{"value": "Scope: \nThis core-EPD relates to 1kg of Sika® ViscoCrete®-6720 (admixture group of Superplasticizers) applied into the building, manufactured at Sikas plant in Domnarvsgatan 15, 163 53 Spnga/ Sweden and is representative for the year 2023.\nThe results in this core-EPD were calculated using an LCA-tool verified by IBU in 2023 \nSystem boundary: \nDeclaration type with respect to life cycle stages covered according to clause 5.2 EN 15804+A2 is cradle to gate with modules C1–C4 and module D (A1–A3, A4, A5, C and D). Modules taken into account:\n• A1: Production of preliminary products\n• A2: Transport to the plant \n• A3: Production including provision of energy, production of auxiliaries and consumables and waste treatment\n• A4: Transport from the construction site to the installation site\n• A5: Installation, admixtures applied into the building during A5 phase operations. At this stage, an impact of the production and treatment of installation residue equal to 1% of the product is considered.\n• C1-C2-C3-C4-D: The building deconstruction (demolition process) takes place in C1 module which considers energy production and consumption in terms of diesel and all the emissions connected with the fuel-burning process. After the demolition, the admixture is transported to the end-of-life processing (C2 module) where all the impacts related to the transport processes are considered. \nC3: Waste processing. No waste processing is considered.One scenario is considered for the final treatment of the waste:100% disposal (C4), modelled by landfill process where admixtures end their life cycle.\nModule D accounts for benefits that are beyond the defined system boundaries. Credits are generated during the incineration of the installation scrap in module A5.", "lang": "en"}, {"value": "Gültigkeitsbereich: \nDiese Kern-EPD bezieht sich auf 1 kg Sika® ViscoCrete®-6720 (Zusatzmittelgruppe der Fließmittel), das im Sika-Werk in Domnarvsgatan 15, 163 53 Spånga/Schweden hergestellt wurde und für das Jahr 2023 repräsentativ ist. Die Ergebnisse in dieser Kern-EPD wurden mit einem von IBU verifizierten LCA-Tool im Jahr 2023 berechnet. \nSystemgrenze: \nDer Deklarationstyp in Bezug auf die gemäß Abschnitt 5.2 EN 15804+A2 abgedeckten Lebenszyklusstadien ist Cradle to Gate mit den Modulen C1-C4 und Modul D (A1-A3, A4, A5, C und D). Berücksichtigte Module: - A1 Produktion von Vorprodukten - A2 Transport zum Werk - A3 Produktion einschließlich Energiebereitstellung, Produktion von Hilfs- und Betriebsstoffen und Abfallbehandlung - A4 Transport von der Baustelle zum Einbauort - A5 Einbau, Zusatzmittel, die während der Phase A5 in das Gebäude eingebracht werden. In dieser Phase wird eine Auswirkung der Produktion und Behandlung von Installationsrückständen in Höhe von 1 % des Produkts berücksichtigt - C1-C2-C4-D Der Rückbau des Gebäudes (Abriss) findet im Modul C1 statt, das die Energieproduktion und den Energieverbrauch in Form von Diesel und alle mit dem Verbrennungsprozess verbundenen Emissionen berücksichtigt. Nach dem Abriss wird das Zusatzmittel zur End-of-Life-Verarbeitung (Modul C2) transportiert, wo alle Auswirkungen im Zusammenhang mit den Transportprozessen berücksichtigt werden. Für die Endbehandlung des Abfalls wird ein Szenario in Betracht gezogen: - 100%ige Entsorgung (C4), modelliert durch den Deponieprozess, bei dem das Zusatzmittel seinen Lebenszyklus beendet. Modul D berücksichtigt Vorteile, die über die definierten Systemgrenzen hinausgehen. Gutschriften werden bei der Verbrennung des Anlagenschrotts in Modul A5 generiert.", "lang": "de"}], "other": {"anies": [{"name": "referenceToOriginalEPD", "value": {"shortDescription": {"value": "Sika® ViscoCrete®-6720.pdf", "defaultValue": "Sika® ViscoCrete®-6720.pdf", "lstrings": [{"lang": "en", "value": "Sika® ViscoCrete®-6720.pdf"}]}, "type": "source data set", "uuid": {"uuid": "1939fc5a-6029-4c82-922f-ba54bb110fee"}, "refObjectId": "1939fc5a-6029-4c82-922f-ba54bb110fee", "resourceURLs": ["https://oekobaudat.de/OEKOBAU.DAT/resource/sources/1939fc5a-6029-4c82-922f-ba54bb110fee/Sika_ViscoCrete-6720_23355.pdf?version=00.03.000"]}}]}}, "validation": {"review": [{"referenceToNameOfReviewerAndInstitution": [{"shortDescription": [{"value": "Institut Bauen und Umwelt e. V.", "lang": "en"}], "type": "contact data set", "refObjectId": "d111dbec-b024-4be5-86c5-752d6eb2cf95", "uri": "../contacts/d111dbec-b024-4be5-86c5-752d6eb2cf95.xml"}], "type": "Accredited third party review"}]}, "complianceDeclarations": {"compliance": [{"referenceToComplianceSystem": {"shortDescription": [{"value": "DIN EN 15804+A2", "lang": "en"}], "type": "source data set", "refObjectId": "c0016b33-8cf7-415c-ac6e-deba0d21440d", "uri": "../sources/c0016b33-8cf7-415c-ac6e-deba0d21440d.xml"}}, {"referenceToComplianceSystem": {"shortDescription": [{"value": "ISO 14025", "lang": "en"}], "type": "source data set", "refObjectId": "4f2eb655-6e44-4874-a95a-e28f5442cd4d", "uri": "../sources/4f2eb655-6e44-4874-a95a-e28f5442cd4d.xml"}}]}}, "administrativeInformation": {"commissionerAndGoal": {"referenceToCommissioner": [{"shortDescription": [{"value": "Sika Sverige AB", "lang": "en"}], "type": "contact data set", "refObjectId": "9ca02c80-c3a3-4ddc-a3ea-976bc3d9545f", "uri": "../contacts/9ca02c80-c3a3-4ddc-a3ea-976bc3d9545f.xml"}]}, "dataGenerator": {"referenceToPersonOrEntityGeneratingTheDataSet": [{"shortDescription": [{"value": "Sika Sverige AB", "lang": "en"}], "type": "contact data set", "refObjectId": "9ca02c80-c3a3-4ddc-a3ea-976bc3d9545f", "uri": "../contacts/9ca02c80-c3a3-4ddc-a3ea-976bc3d9545f.xml"}]}, "dataEntryBy": {"timeStamp": 1737504000000, "referenceToDataSetFormat": [{"shortDescription": [{"value": "ILCD Format", "lang": "en"}], "type": "source data set", "refObjectId": "a97a0155-0234-4b87-b4ce-a45da52f2a40", "uri": "../sources/a97a0155-0234-4b87-b4ce-a45da52f2a40.xml"}, {"shortDescription": [{"value": "EPD-Datenformaterweiterungen v1.2", "lang": "de"}, {"value": "EPD Data Format Extensions v1.2", "lang": "en"}], "type": "source data set", "refObjectId": "a29449fd-aa2f-4de8-b5d7-4b06b43c6fde", "uri": "../sources/a29449fd-aa2f-4de8-b5d7-4b06b43c6fde.xml"}]}, "publicationAndOwnership": {"dataSetVersion": "00.04.000", "referenceToRegistrationAuthority": {"shortDescription": [{"value": "Institut Bauen und Umwelt e. V.", "lang": "en"}], "type": "contact data set", "refObjectId": "d111dbec-b024-4be5-86c5-752d6eb2cf95", "uri": "../contacts/d111dbec-b024-4be5-86c5-752d6eb2cf95.xml"}, "registrationNumber": "EPD-SIK-20240397-CBA3-EN", "referenceToOwnershipOfDataSet": {"shortDescription": [{"value": "Sika Sverige AB", "lang": "en"}], "type": "contact data set", "refObjectId": "9ca02c80-c3a3-4ddc-a3ea-976bc3d9545f", "uri": "../contacts/9ca02c80-c3a3-4ddc-a3ea-976bc3d9545f.xml"}, "copyright": true, "licenseType": "Free of charge for all users and uses", "accessRestrictions": [{"value": "None", "lang": "en"}], "other": {"anies": [{"name": "referenceToPublisher", "value": {"shortDescription": [{"value": "Institut Bauen und Umwelt e. V.", "lang": "en"}], "type": "contact data set", "refObjectId": "d111dbec-b024-4be5-86c5-752d6eb2cf95", "uri": "../contacts/d111dbec-b024-4be5-86c5-752d6eb2cf95.xml"}}]}}}, "exchanges": {"exchange": [{"dataSetInternalID": 0, "referenceToFlowDataSet": {"shortDescription": [{"value": "Sika® ViscoCrete®-6720 (Sika® ViscoCrete®-6720)", "lang": "en"}], "type": "flow data set", "refObjectId": "9e7ecf33-f477-2d39-a52c-e531b786906a", "uri": "../flows/9e7ecf33-f477-2d39-a52c-e531b786906a.xml"}, "meanAmount": 1.0, "referencesToDataSource": {}, "referenceFlow": true, "resolvedFlowVersion": "00.04.000", "resultingflowAmount": 1.0, "flowProperties": [{"name": [{"lang": "en", "value": "Mass"}, {"lang": "de", "value": "Masse"}], "uuid": "93a60a56-a3c8-11da-a746-0800200b9a66", "referenceFlowProperty": true, "meanValue": 1.0, "referenceUnit": "kg", "unitGroupUUID": "ad38d542-3fe9-439d-9b95-2f5f7752acaf"}], "materialProperties": [{"name": "gross density", "value": "1.03", "unit": "kg/m^3", "unitDescription": "kilograms per cubic metre"}], "typeOfFlow": "Product flow", "classification": {"classHierarchy": "Mineralische Baustoffe / Mörtel und Beton / Betonzusatzmittel", "name": "OEKOBAU.DAT"}}, {"dataSetInternalID": 1, "referenceToFlowDataSet": {"shortDescription": [{"value": "Renewable primary energy as energy carrier (PERE)", "lang": "en"}, {"value": "Erneuerbare Primärenergie als Energieträger (PERE)", "lang": "de"}], "type": "flow data set", "refObjectId": "20f32be5-0398-4288-9b6d-accddd195317", "uri": "../flows/20f32be5-0398-4288-9b6d-accddd195317.xml"}, "exchange direction": "INPUT", "other": {"anies": [{"name": "referenceToUnitGroupDataSet", "value": {"shortDescription": [{"value": "MJ", "lang": "en"}], "type": "unit group data set", "refObjectId": "93a60a57-a3c8-11da-a746-0800200c9a66", "uri": "../unitgroups/93a60a57-a3c8-11da-a746-0800200c9a66.xml"}}, {"value": "0.865615217881892", "module": "A1-A3"}, {"value": "0.00193978013047042", "module": "A4"}, {"value": "0.00968005354222721", "module": "A5"}, {"value": "2.32553988538965E-05", "module": "C1"}, {"value": "0.000507674173931432", "module": "C2"}, {"value": "0", "module": "C3"}, {"value": "0.0293410292280937", "module": "C4"}, {"value": "-0.0128137371987978", "module": "D"}]}, "resolvedFlowVersion": "38.00.000", "flowProperties": [], "typeOfFlow": "Other flow", "classification": {"classHierarchy": "Quantities", "name": "GaBiCategories"}}, {"dataSetInternalID": 2, "referenceToFlowDataSet": {"shortDescription": [{"value": "Renewable primary energy resources as material utilization (PERM)", "lang": "en"}, {"value": "Erneuerbare Primärenergie zur stofflichen Nutzung (PERM)", "lang": "de"}], "type": "flow data set", "refObjectId": "fb3ec0de-548d-4508-aea5-00b73bf6f702", "uri": "../flows/fb3ec0de-548d-4508-aea5-00b73bf6f702.xml"}, "exchange direction": "INPUT", "other": {"anies": [{"name": "referenceToUnitGroupDataSet", "value": {"shortDescription": [{"value": "MJ", "lang": "en"}], "type": "unit group data set", "refObjectId": "93a60a57-a3c8-11da-a746-0800200c9a66", "uri": "../unitgroups/93a60a57-a3c8-11da-a746-0800200c9a66.xml"}}, {"value": "0", "module": "A1-A3"}, {"value": "0", "module": "A4"}, {"value": "0", "module": "A5"}, {"value": "0", "module": "C1"}, {"value": "0", "module": "C2"}, {"value": "0", "module": "C3"}, {"value": "0", "module": "C4"}, {"value": "0", "module": "D"}]}, "resolvedFlowVersion": "38.00.000", "flowProperties": [], "typeOfFlow": "Other flow", "classification": {"classHierarchy": "Quantities", "name": "GaBiCategories"}}, {"dataSetInternalID": 3, "referenceToFlowDataSet": {"shortDescription": [{"value": "Total use of renewable primary energy resources (PERT)", "lang": "en"}, {"value": "Total erneuerbare Primärenergie (PERT)", "lang": "de"}], "type": "flow data set", "refObjectId": "53f97275-fa8a-4cdd-9024-65936002acd0", "uri": "../flows/53f97275-fa8a-4cdd-9024-65936002acd0.xml"}, "exchange direction": "INPUT", "other": {"anies": [{"name": "referenceToUnitGroupDataSet", "value": {"shortDescription": [{"value": "MJ", "lang": "en"}], "type": "unit group data set", "refObjectId": "93a60a57-a3c8-11da-a746-0800200c9a66", "uri": "../unitgroups/93a60a57-a3c8-11da-a746-0800200c9a66.xml"}}, {"value": "0.865615217881892", "module": "A1-A3"}, {"value": "0.00193978013047042", "module": "A4"}, {"value": "0.00968005354222721", "module": "A5"}, {"value": "2.32553988538965E-05", "module": "C1"}, {"value": "0.000507674173931432", "module": "C2"}, {"value": "0", "module": "C3"}, {"value": "0.0293410292280937", "module": "C4"}, {"value": "-0.0128137371987978", "module": "D"}]}, "resolvedFlowVersion": "38.00.000", "flowProperties": [], "typeOfFlow": "Other flow", "classification": {"classHierarchy": "Quantities / Environmental quantities / EPD EN 15804 / LCI indicators", "name": "GaBiCategories"}}, {"dataSetInternalID": 4, "referenceToFlowDataSet": {"shortDescription": [{"value": "Non renewable primary energy as energy carrier (PENRE)", "lang": "en"}, {"value": "Nicht-erneuerbare Primärenergie als Energieträger (PENRE)", "lang": "de"}], "type": "flow data set", "refObjectId": "ac857178-2b45-46ec-892a-a9a4332f0372", "uri": "../flows/ac857178-2b45-46ec-892a-a9a4332f0372.xml"}, "exchange direction": "INPUT", "other": {"anies": [{"name": "referenceToUnitGroupDataSet", "value": {"shortDescription": [{"value": "MJ", "lang": "en"}], "type": "unit group data set", "refObjectId": "93a60a57-a3c8-11da-a746-0800200c9a66", "uri": "../unitgroups/93a60a57-a3c8-11da-a746-0800200c9a66.xml"}}, {"value": "6.90186139197613", "module": "A1-A3"}, {"value": "0.321733985916552", "module": "A4"}, {"value": "0.125278943205656", "module": "A5"}, {"value": "0.00385716507237801", "module": "C1"}, {"value": "0.0842033759188171", "module": "C2"}, {"value": "0", "module": "C3"}, {"value": "0.195734599865599", "module": "C4"}, {"value": "-0.0529241999361442", "module": "D"}]}, "resolvedFlowVersion": "38.00.000", "flowProperties": [], "typeOfFlow": "Other flow", "classification": {"classHierarchy": "Quantities", "name": "GaBiCategories"}}, {"dataSetInternalID": 5, "referenceToFlowDataSet": {"shortDescription": [{"value": "Non renewable primary energy as material utilization (PENRM)", "lang": "en"}, {"value": "Nicht-erneuerbare Primärenergie zur stofflichen Nutzung (PENRM)", "lang": "de"}], "type": "flow data set", "refObjectId": "1421caa0-679d-4bf4-b282-0eb850ccae27", "uri": "../flows/1421caa0-679d-4bf4-b282-0eb850ccae27.xml"}, "exchange direction": "INPUT", "other": {"anies": [{"name": "referenceToUnitGroupDataSet", "value": {"shortDescription": [{"value": "MJ", "lang": "en"}], "type": "unit group data set", "refObjectId": "93a60a57-a3c8-11da-a746-0800200c9a66", "uri": "../unitgroups/93a60a57-a3c8-11da-a746-0800200c9a66.xml"}}, {"value": "4.82", "module": "A1-A3"}, {"value": "0", "module": "A4"}, {"value": "0", "module": "A5"}, {"value": "0", "module": "C1"}, {"value": "0", "module": "C2"}, {"value": "0", "module": "C3"}, {"value": "0", "module": "C4"}, {"value": "0", "module": "D"}]}, "resolvedFlowVersion": "38.00.000", "flowProperties": [], "typeOfFlow": "Other flow", "classification": {"classHierarchy": "Quantities", "name": "GaBiCategories"}}, {"dataSetInternalID": 6, "referenceToFlowDataSet": {"shortDescription": [{"value": "Total use of non renewable primary energy resources (PENRT)", "lang": "en"}, {"value": "Total nicht erneuerbare Primärenergie (PENRT)", "lang": "de"}], "type": "flow data set", "refObjectId": "06159210-646b-4c8d-8583-da9b3b95a6c1", "uri": "../flows/06159210-646b-4c8d-8583-da9b3b95a6c1.xml"}, "exchange direction": "INPUT", "other": {"anies": [{"name": "referenceToUnitGroupDataSet", "value": {"shortDescription": [{"value": "MJ", "lang": "en"}], "type": "unit group data set", "refObjectId": "93a60a57-a3c8-11da-a746-0800200c9a66", "uri": "../unitgroups/93a60a57-a3c8-11da-a746-0800200c9a66.xml"}}, {"value": "11.7218613919762", "module": "A1-A3"}, {"value": "0.321733985916552", "module": "A4"}, {"value": "0.125278943205657", "module": "A5"}, {"value": "0.00385716507237801", "module": "C1"}, {"value": "0.0842033759188171", "module": "C2"}, {"value": "0", "module": "C3"}, {"value": "0.1957345998656", "module": "C4"}, {"value": "-0.0529241999361446", "module": "D"}]}, "resolvedFlowVersion": "38.00.000", "flowProperties": [], "typeOfFlow": "Other flow", "classification": {"classHierarchy": "Quantities / Environmental quantities / EPD EN 15804 / LCI indicators", "name": "GaBiCategories"}}, {"dataSetInternalID": 7, "referenceToFlowDataSet": {"shortDescription": [{"value": "Use of secondary material (SM)", "lang": "en"}, {"value": "Einsatz von Sekundärstoffen (SM)", "lang": "de"}], "type": "flow data set", "refObjectId": "c6a1f35f-2d09-4f54-8dfb-97e502e1ce92", "uri": "../flows/c6a1f35f-2d09-4f54-8dfb-97e502e1ce92.xml"}, "exchange direction": "INPUT", "other": {"anies": [{"name": "referenceToUnitGroupDataSet", "value": {"shortDescription": [{"value": "kg", "lang": "en"}], "type": "unit group data set", "refObjectId": "ad38d542-3fe9-439d-9b95-2f5f7752acaf", "uri": "../unitgroups/ad38d542-3fe9-439d-9b95-2f5f7752acaf.xml"}}, {"value": "0", "module": "A1-A3"}, {"value": "0", "module": "A4"}, {"value": "0", "module": "A5"}, {"value": "0", "module": "C1"}, {"value": "0", "module": "C2"}, {"value": "0", "module": "C3"}, {"value": "0", "module": "C4"}, {"value": "0", "module": "D"}]}, "resolvedFlowVersion": "38.00.000", "flowProperties": [], "typeOfFlow": "Other flow", "classification": {"classHierarchy": "Quantities / Environmental quantities / EPD EN 15804 / LCI indicators", "name": "GaBiCategories"}}, {"dataSetInternalID": 8, "referenceToFlowDataSet": {"shortDescription": [{"value": "Use of renewable secondary fuels (RSF)", "lang": "en"}, {"value": "Erneuerbare Sekundärbrennstoffe (RSF)", "lang": "de"}], "type": "flow data set", "refObjectId": "64333088-a55f-4aa2-9a31-c10b07816787", "uri": "../flows/64333088-a55f-4aa2-9a31-c10b07816787.xml"}, "exchange direction": "INPUT", "other": {"anies": [{"name": "referenceToUnitGroupDataSet", "value": {"shortDescription": [{"value": "MJ", "lang": "en"}], "type": "unit group data set", "refObjectId": "93a60a57-a3c8-11da-a746-0800200c9a66", "uri": "../unitgroups/93a60a57-a3c8-11da-a746-0800200c9a66.xml"}}, {"value": "0", "module": "A1-A3"}, {"value": "0", "module": "A4"}, {"value": "0", "module": "A5"}, {"value": "0", "module": "C1"}, {"value": "0", "module": "C2"}, {"value": "0", "module": "C3"}, {"value": "0", "module": "C4"}, {"value": "0", "module": "D"}]}, "resolvedFlowVersion": "38.00.000", "flowProperties": [], "typeOfFlow": "Other flow", "classification": {"classHierarchy": "Quantities / Environmental quantities / EPD EN 15804 / LCI indicators", "name": "GaBiCategories"}}, {"dataSetInternalID": 9, "referenceToFlowDataSet": {"shortDescription": [{"value": "Use of non renewable secondary fuels (NRSF)", "lang": "en"}, {"value": "Nicht erneuerbare Sekundärbrennstoffe (NRSF)", "lang": "de"}], "type": "flow data set", "refObjectId": "89def144-d39a-4287-b86f-efde453ddcb2", "uri": "../flows/89def144-d39a-4287-b86f-efde453ddcb2.xml"}, "exchange direction": "INPUT", "other": {"anies": [{"name": "referenceToUnitGroupDataSet", "value": {"shortDescription": [{"value": "MJ", "lang": "en"}], "type": "unit group data set", "refObjectId": "93a60a57-a3c8-11da-a746-0800200c9a66", "uri": "../unitgroups/93a60a57-a3c8-11da-a746-0800200c9a66.xml"}}, {"value": "0", "module": "A1-A3"}, {"value": "0", "module": "A4"}, {"value": "0", "module": "A5"}, {"value": "0", "module": "C1"}, {"value": "0", "module": "C2"}, {"value": "0", "module": "C3"}, {"value": "0", "module": "C4"}, {"value": "0", "module": "D"}]}, "resolvedFlowVersion": "38.00.000", "flowProperties": [], "typeOfFlow": "Other flow", "classification": {"classHierarchy": "Quantities / Environmental quantities / EPD EN 15804 / LCI indicators", "name": "GaBiCategories"}}, {"dataSetInternalID": 10, "referenceToFlowDataSet": {"shortDescription": [{"value": "Use of net fresh water (FW)", "lang": "en"}, {"value": "Einsatz von Süßwasserressourcen (FW)", "lang": "de"}], "type": "flow data set", "refObjectId": "3cf952c8-f3a4-461d-8c96-96456ca62246", "uri": "../flows/3cf952c8-f3a4-461d-8c96-96456ca62246.xml"}, "exchange direction": "INPUT", "other": {"anies": [{"name": "referenceToUnitGroupDataSet", "value": {"shortDescription": [{"value": "m^3", "lang": "en"}], "type": "unit group data set", "refObjectId": "cd950537-0a98-4044-9ba7-9f9a68d0a504", "uri": "../unitgroups/cd950537-0a98-4044-9ba7-9f9a68d0a504.xml"}}, {"value": "0.00417262423016656", "module": "A1-A3"}, {"value": "2.63577197457553E-06", "module": "A4"}, {"value": "7.84609225442016E-05", "module": "A5"}, {"value": "3.15994207765246E-08", "module": "C1"}, {"value": "6.89827336018617E-07", "module": "C2"}, {"value": "0", "module": "C3"}, {"value": "4.96705824522798E-05", "module": "C4"}, {"value": "-1.23432009457094E-05", "module": "D"}]}, "resolvedFlowVersion": "38.00.000", "flowProperties": [], "typeOfFlow": "Other flow", "classification": {"classHierarchy": "Quantities / Environmental quantities / EPD EN 15804 / LCI indicators", "name": "GaBiCategories"}}, {"dataSetInternalID": 11, "referenceToFlowDataSet": {"shortDescription": [{"value": "Hazardous waste disposed (HWD)", "lang": "en"}, {"value": "Gefährlicher Abfall zur Deponie (HWD)", "lang": "de"}], "type": "flow data set", "refObjectId": "430f9e0f-59b2-46a0-8e0d-55e0e84948fc", "uri": "../flows/430f9e0f-59b2-46a0-8e0d-55e0e84948fc.xml"}, "exchange direction": "OUTPUT", "other": {"anies": [{"name": "referenceToUnitGroupDataSet", "value": {"shortDescription": [{"value": "kg", "lang": "en"}], "type": "unit group data set", "refObjectId": "ad38d542-3fe9-439d-9b95-2f5f7752acaf", "uri": "../unitgroups/ad38d542-3fe9-439d-9b95-2f5f7752acaf.xml"}}, {"value": "5.9689480630675E-10", "module": "A1-A3"}, {"value": "1.11048826511875E-12", "module": "A4"}, {"value": "6.4572229466321E-12", "module": "A5"}, {"value": "1.33132859349608E-14", "module": "C1"}, {"value": "2.90634079501574E-13", "module": "C2"}, {"value": "0", "module": "C3"}, {"value": "1.00516082523196E-11", "module": "C4"}, {"value": "-7.46468626489312E-12", "module": "D"}]}, "resolvedFlowVersion": "38.00.000", "flowProperties": [], "typeOfFlow": "Other flow", "classification": {"classHierarchy": "Quantities / Environmental quantities / EPD EN 15804 / LCI indicators", "name": "GaBiCategories"}}, {"dataSetInternalID": 12, "referenceToFlowDataSet": {"shortDescription": [{"value": "Non hazardous waste disposed (NHWD)", "lang": "en"}, {"value": "Entsorgter nicht gefährlicher Abfall (NHWD)", "lang": "de"}], "type": "flow data set", "refObjectId": "b29ef66b-e286-4afa-949f-62f1a7b4d7fa", "uri": "../flows/b29ef66b-e286-4afa-949f-62f1a7b4d7fa.xml"}, "exchange direction": "OUTPUT", "other": {"anies": [{"name": "referenceToUnitGroupDataSet", "value": {"shortDescription": [{"value": "kg", "lang": "en"}], "type": "unit group data set", "refObjectId": "ad38d542-3fe9-439d-9b95-2f5f7752acaf", "uri": "../unitgroups/ad38d542-3fe9-439d-9b95-2f5f7752acaf.xml"}}, {"value": "0.0112880225400003", "module": "A1-A3"}, {"value": "3.28497884996002E-05", "module": "A4"}, {"value": "0.00126749766591385", "module": "A5"}, {"value": "3.93825527864895E-07", "module": "C1"}, {"value": "8.59736058659001E-06", "module": "C2"}, {"value": "0", "module": "C3"}, {"value": "1.00098433405176", "module": "C4"}, {"value": "-2.52165731550572E-05", "module": "D"}]}, "resolvedFlowVersion": "38.00.000", "flowProperties": [], "typeOfFlow": "Other flow", "classification": {"classHierarchy": "Quantities / Environmental quantities / EPD EN 15804 / LCI indicators", "name": "GaBiCategories"}}, {"dataSetInternalID": 13, "referenceToFlowDataSet": {"shortDescription": [{"value": "Radioactive waste disposed (RWD)", "lang": "en"}, {"value": "Entsorgter radioaktiver Abfall (RWD)", "lang": "de"}], "type": "flow data set", "refObjectId": "3449546e-52ad-4b39-b809-9fb77cea8ff6", "uri": "../flows/3449546e-52ad-4b39-b809-9fb77cea8ff6.xml"}, "exchange direction": "OUTPUT", "other": {"anies": [{"name": "referenceToUnitGroupDataSet", "value": {"shortDescription": [{"value": "kg", "lang": "en"}], "type": "unit group data set", "refObjectId": "ad38d542-3fe9-439d-9b95-2f5f7752acaf", "uri": "../unitgroups/ad38d542-3fe9-439d-9b95-2f5f7752acaf.xml"}}, {"value": "0.00044238049526285", "module": "A1-A3"}, {"value": "5.30361989544241E-07", "module": "A4"}, {"value": "4.6642420119514E-06", "module": "A5"}, {"value": "6.35833897360644E-09", "module": "C1"}, {"value": "1.38804950466838E-07", "module": "C2"}, {"value": "0", "module": "C3"}, {"value": "2.1781577410322E-06", "module": "C4"}, {"value": "-3.67031631519383E-06", "module": "D"}]}, "resolvedFlowVersion": "38.00.000", "flowProperties": [], "typeOfFlow": "Other flow", "classification": {"classHierarchy": "Quantities / Environmental quantities / EPD EN 15804 / LCI indicators", "name": "GaBiCategories"}}, {"dataSetInternalID": 14, "referenceToFlowDataSet": {"shortDescription": [{"value": "Components for re-use (CRU)", "lang": "en"}, {"value": "Komponenten für die Wiederverwendung (CRU)", "lang": "de"}], "type": "flow data set", "refObjectId": "a2b32f97-3fc7-4af2-b209-525bc6426f33", "uri": "../flows/a2b32f97-3fc7-4af2-b209-525bc6426f33.xml"}, "exchange direction": "OUTPUT", "other": {"anies": [{"name": "referenceToUnitGroupDataSet", "value": {"shortDescription": [{"value": "kg", "lang": "en"}], "type": "unit group data set", "refObjectId": "ad38d542-3fe9-439d-9b95-2f5f7752acaf", "uri": "../unitgroups/ad38d542-3fe9-439d-9b95-2f5f7752acaf.xml"}}, {"value": "0", "module": "A1-A3"}, {"value": "0", "module": "A4"}, {"value": "0", "module": "A5"}, {"value": "0", "module": "C1"}, {"value": "0", "module": "C2"}, {"value": "0", "module": "C3"}, {"value": "0", "module": "C4"}, {"value": "0", "module": "D"}]}, "resolvedFlowVersion": "38.00.000", "flowProperties": [], "typeOfFlow": "Other flow", "classification": {"classHierarchy": "Quantities / Environmental quantities / EPD EN 15804 / LCI indicators", "name": "GaBiCategories"}}, {"dataSetInternalID": 15, "referenceToFlowDataSet": {"shortDescription": [{"value": "Materials for recycling (MFR)", "lang": "en"}, {"value": "Stoffe zum Recycling (MFR)", "lang": "de"}], "type": "flow data set", "refObjectId": "d7fe48a5-4103-49c8-9aae-b0b5dfdbd6ae", "uri": "../flows/d7fe48a5-4103-49c8-9aae-b0b5dfdbd6ae.xml"}, "exchange direction": "OUTPUT", "other": {"anies": [{"name": "referenceToUnitGroupDataSet", "value": {"shortDescription": [{"value": "kg", "lang": "en"}], "type": "unit group data set", "refObjectId": "ad38d542-3fe9-439d-9b95-2f5f7752acaf", "uri": "../unitgroups/ad38d542-3fe9-439d-9b95-2f5f7752acaf.xml"}}, {"value": "0", "module": "A1-A3"}, {"value": "0", "module": "A4"}, {"value": "0", "module": "A5"}, {"value": "0", "module": "C1"}, {"value": "0", "module": "C2"}, {"value": "0", "module": "C3"}, {"value": "0", "module": "C4"}, {"value": "0", "module": "D"}]}, "resolvedFlowVersion": "38.00.000", "flowProperties": [], "typeOfFlow": "Other flow", "classification": {"classHierarchy": "Quantities / Environmental quantities / EPD EN 15804 / LCI indicators", "name": "GaBiCategories"}}, {"dataSetInternalID": 16, "referenceToFlowDataSet": {"shortDescription": [{"value": "Materials for energy recovery (MER)", "lang": "en"}, {"value": "Stoffe für die Energierückgewinnung (MER)", "lang": "de"}], "type": "flow data set", "refObjectId": "59a9181c-3aaf-46ee-8b13-2b3723b6e447", "uri": "../flows/59a9181c-3aaf-46ee-8b13-2b3723b6e447.xml"}, "exchange direction": "OUTPUT", "other": {"anies": [{"name": "referenceToUnitGroupDataSet", "value": {"shortDescription": [{"value": "kg", "lang": "en"}], "type": "unit group data set", "refObjectId": "ad38d542-3fe9-439d-9b95-2f5f7752acaf", "uri": "../unitgroups/ad38d542-3fe9-439d-9b95-2f5f7752acaf.xml"}}, {"value": "0", "module": "A1-A3"}, {"value": "0", "module": "A4"}, {"value": "0", "module": "A5"}, {"value": "0", "module": "C1"}, {"value": "0", "module": "C2"}, {"value": "0", "module": "C3"}, {"value": "0", "module": "C4"}, {"value": "0", "module": "D"}]}, "resolvedFlowVersion": "38.00.000", "flowProperties": [], "typeOfFlow": "Other flow", "classification": {"classHierarchy": "Quantities / Environmental quantities / EPD EN 15804 / LCI indicators", "name": "GaBiCategories"}}, {"dataSetInternalID": 17, "referenceToFlowDataSet": {"shortDescription": [{"value": "Exported electrical energy (EEE)", "lang": "en"}, {"value": "Exportierte elektrische Energie (EEE)", "lang": "de"}], "type": "flow data set", "refObjectId": "4da0c987-2b76-40d6-9e9e-82a017aaaf29", "uri": "../flows/4da0c987-2b76-40d6-9e9e-82a017aaaf29.xml"}, "exchange direction": "OUTPUT", "other": {"anies": [{"name": "referenceToUnitGroupDataSet", "value": {"shortDescription": [{"value": "MJ", "lang": "en"}], "type": "unit group data set", "refObjectId": "93a60a57-a3c8-11da-a746-0800200c9a66", "uri": "../unitgroups/93a60a57-a3c8-11da-a746-0800200c9a66.xml"}}, {"value": "0", "module": "A1-A3"}, {"value": "0", "module": "A4"}, {"value": "0.0123153588664162", "module": "A5"}, {"value": "0", "module": "C1"}, {"value": "0", "module": "C2"}, {"value": "0", "module": "C3"}, {"value": "0", "module": "C4"}, {"value": "0", "module": "D"}]}, "resolvedFlowVersion": "38.00.000", "flowProperties": [], "typeOfFlow": "Other flow", "classification": {"classHierarchy": "Quantities / Environmental quantities / EPD EN 15804 / LCI indicators", "name": "GaBiCategories"}}, {"dataSetInternalID": 18, "referenceToFlowDataSet": {"shortDescription": [{"value": "Exported thermal energy (EET)", "lang": "en"}, {"value": "Exportierte thermische Energie (EET)", "lang": "de"}], "type": "flow data set", "refObjectId": "98daf38a-7a79-46d3-9a37-2b7bd0955810", "uri": "../flows/98daf38a-7a79-46d3-9a37-2b7bd0955810.xml"}, "exchange direction": "OUTPUT", "other": {"anies": [{"name": "referenceToUnitGroupDataSet", "value": {"shortDescription": [{"value": "MJ", "lang": "en"}], "type": "unit group data set", "refObjectId": "93a60a57-a3c8-11da-a746-0800200c9a66", "uri": "../unitgroups/93a60a57-a3c8-11da-a746-0800200c9a66.xml"}}, {"value": "0", "module": "A1-A3"}, {"value": "0", "module": "A4"}, {"value": "0.0280695829618573", "module": "A5"}, {"value": "0", "module": "C1"}, {"value": "0", "module": "C2"}, {"value": "0", "module": "C3"}, {"value": "0", "module": "C4"}, {"value": "0", "module": "D"}]}, "resolvedFlowVersion": "38.00.000", "flowProperties": [], "typeOfFlow": "Other flow", "classification": {"classHierarchy": "Quantities / Environmental quantities / EPD EN 15804 / LCI indicators", "name": "GaBiCategories"}}]}, "LCIAResults": {"LCIAResult": [{"referenceToLCIAMethodDataSet": {"shortDescription": [{"value": "Global Warming Potential total (GWP-total)", "lang": "en"}, {"value": "Globales Erwärmungspotenzial total (GWP-total)", "lang": "de"}], "type": "LCIA method data set", "refObjectId": "6a37f984-a4b3-458a-a20a-64418c145fa2", "uri": "../lciamethods/6a37f984-a4b3-458a-a20a-64418c145fa2.xml"}, "other": {"anies": [{"name": "referenceToUnitGroupDataSet", "value": {"shortDescription": [{"value": "kg CO_(2) eq", "lang": "en"}], "type": "unit group data set", "refObjectId": "1ebf3012-d0db-4de2-aefd-ef30cedb0be1", "uri": "../unitgroups/1ebf3012-d0db-4de2-aefd-ef30cedb0be1.xml"}}, {"value": "0.372064893972701", "module": "A1-A3"}, {"value": "0.0239091304498285", "module": "A4"}, {"value": "0.0133553654227182", "module": "A5"}, {"value": "0.000282518721608003", "module": "C1"}, {"value": "0.0062739468259078", "module": "C2"}, {"value": "0", "module": "C3"}, {"value": "0.0145083160010643", "module": "C4"}, {"value": "-0.00314897328301095", "module": "D"}]}}, {"referenceToLCIAMethodDataSet": {"shortDescription": [{"value": "Global Warming Potential fossil fuels (GWP-fossil)", "lang": "en"}, {"value": "Globales Erwärmungspotenzial fossil (GWP-fossil)", "lang": "de"}], "type": "LCIA method data set", "refObjectId": "5f635281-343e-44fb-83df-1971b155e6b6", "uri": "../lciamethods/5f635281-343e-44fb-83df-1971b155e6b6.xml"}, "other": {"anies": [{"name": "referenceToUnitGroupDataSet", "value": {"shortDescription": [{"value": "kg CO_(2) eq", "lang": "en"}], "type": "unit group data set", "refObjectId": "1ebf3012-d0db-4de2-aefd-ef30cedb0be1", "uri": "../unitgroups/1ebf3012-d0db-4de2-aefd-ef30cedb0be1.xml"}}, {"value": "0.36377292779505", "module": "A1-A3"}, {"value": "0.0228739716809874", "module": "A4"}, {"value": "0.00810914770552166", "module": "A5"}, {"value": "0.000270173798366767", "module": "C1"}, {"value": "0.0060030277755249", "module": "C2"}, {"value": "0", "module": "C3"}, {"value": "0.0149229433380744", "module": "C4"}, {"value": "-0.00313394579106055", "module": "D"}]}}, {"referenceToLCIAMethodDataSet": {"shortDescription": [{"value": "Global Warming Potential biogenic (GWP-biogenic)", "lang": "en"}, {"value": "Globales Erwärmungspotenzial biogen (GWP-biogenic)", "lang": "de"}], "type": "LCIA method data set", "refObjectId": "2356e1ab-0185-4db5-86e5-16de51c7485c", "uri": "../lciamethods/2356e1ab-0185-4db5-86e5-16de51c7485c.xml"}, "other": {"anies": [{"name": "referenceToUnitGroupDataSet", "value": {"shortDescription": [{"value": "kg CO_(2) eq", "lang": "en"}], "type": "unit group data set", "refObjectId": "1ebf3012-d0db-4de2-aefd-ef30cedb0be1", "uri": "../unitgroups/1ebf3012-d0db-4de2-aefd-ef30cedb0be1.xml"}}, {"value": "0.00825539978757498", "module": "A1-A3"}, {"value": "0.00103411798372421", "module": "A4"}, {"value": "0.00524589838937653", "module": "A5"}, {"value": "1.23324456038817E-05", "module": "C1"}, {"value": "0.000270646658828742", "module": "C2"}, {"value": "0", "module": "C3"}, {"value": "-0.000442172461500264", "module": "C4"}, {"value": "-1.47173139761128E-05", "module": "D"}]}}, {"referenceToLCIAMethodDataSet": {"shortDescription": [{"value": "Global Warming Potential luluc (GWP-luluc)", "lang": "en"}, {"value": "Globales Erwärmungspotenzial luluc (GWP-luluc)", "lang": "de"}], "type": "LCIA method data set", "refObjectId": "4331bbdb-978a-490d-8707-eeb047f01a55", "uri": "../lciamethods/4331bbdb-978a-490d-8707-eeb047f01a55.xml"}, "other": {"anies": [{"name": "referenceToUnitGroupDataSet", "value": {"shortDescription": [{"value": "kg CO_(2) eq", "lang": "en"}], "type": "unit group data set", "refObjectId": "1ebf3012-d0db-4de2-aefd-ef30cedb0be1", "uri": "../unitgroups/1ebf3012-d0db-4de2-aefd-ef30cedb0be1.xml"}}, {"value": "3.65663900746589E-05", "module": "A1-A3"}, {"value": "1.04078511689621E-06", "module": "A4"}, {"value": "3.19327820038037E-07", "module": "A5"}, {"value": "1.24776373540598E-08", "module": "C1"}, {"value": "2.72391554156333E-07", "module": "C2"}, {"value": "0", "module": "C3"}, {"value": "2.7545124490233E-05", "module": "C4"}, {"value": "-3.10177974287926E-07", "module": "D"}]}}, {"referenceToLCIAMethodDataSet": {"shortDescription": [{"value": "Depletion potential of the stratospheric ozone layer (ODP)", "lang": "en"}, {"value": "Abbau Potential der stratosphärischen Ozonschicht (ODP)", "lang": "de"}], "type": "LCIA method data set", "refObjectId": "b5c629d6-def3-11e6-bf01-fe55135034f3", "uri": "../lciamethods/b5c629d6-def3-11e6-bf01-fe55135034f3.xml"}, "other": {"anies": [{"name": "referenceToUnitGroupDataSet", "value": {"shortDescription": [{"value": "kg CFC11 eq", "lang": "en"}], "type": "unit group data set", "refObjectId": "d9e957c9-7309-4474-bf3a-7777df6c4e5b", "uri": "../unitgroups/d9e957c9-7309-4474-bf3a-7777df6c4e5b.xml"}}, {"value": "1.16852499870093E-12", "module": "A1-A3"}, {"value": "2.34898825166145E-15", "module": "A4"}, {"value": "1.34993038053575E-14", "module": "A5"}, {"value": "2.81612631439093E-17", "module": "C1"}, {"value": "6.14771051370479E-16", "module": "C2"}, {"value": "0", "module": "C3"}, {"value": "3.5078861858161E-14", "module": "C4"}, {"value": "-1.85290629114898E-14", "module": "D"}]}}, {"referenceToLCIAMethodDataSet": {"shortDescription": [{"value": "Acidification potential of land and water (AP)", "lang": "en"}, {"value": "Versauerungspotenzial von Boden und Wasser (AP)", "lang": "de"}], "type": "LCIA method data set", "refObjectId": "b5c611c6-def3-11e6-bf01-fe55135034f3", "uri": "../lciamethods/b5c611c6-def3-11e6-bf01-fe55135034f3.xml"}, "other": {"anies": [{"name": "referenceToUnitGroupDataSet", "value": {"shortDescription": [{"value": "mol H^(+) eq", "lang": "en"}], "type": "unit group data set", "refObjectId": "42e089ac-92bf-4bf2-8ca1-5fc40d18f2ed", "uri": "../unitgroups/42e089ac-92bf-4bf2-8ca1-5fc40d18f2ed.xml"}}, {"value": "0.000760190376564231", "module": "A1-A3"}, {"value": "6.66907831544594E-05", "module": "A4"}, {"value": "1.28972101849872E-05", "module": "A5"}, {"value": "3.6236464398103E-06", "module": "C1"}, {"value": "1.91101914625367E-05", "module": "C2"}, {"value": "0", "module": "C3"}, {"value": "0.000105799899434752", "module": "C4"}, {"value": "-3.82538883559353E-06", "module": "D"}]}}, {"referenceToLCIAMethodDataSet": {"shortDescription": [{"value": "Eutrophication potential aquatic freshwater (EP-freshwater)", "lang": "en"}, {"value": "Eutrophierungspotenzial Süßwasser (EP-freshwater)", "lang": "de"}], "type": "LCIA method data set", "refObjectId": "b53ec18f-7377-4ad3-86eb-cc3f4f276b2b", "uri": "../lciamethods/b53ec18f-7377-4ad3-86eb-cc3f4f276b2b.xml"}, "other": {"anies": [{"name": "referenceToUnitGroupDataSet", "value": {"shortDescription": [{"value": "kg P eq", "lang": "en"}], "type": "unit group data set", "refObjectId": "0429039d-a61d-4590-ba67-aa4a20a810a1", "uri": "../unitgroups/0429039d-a61d-4590-ba67-aa4a20a810a1.xml"}}, {"value": "2.81929247207615E-06", "module": "A1-A3"}, {"value": "5.34925820501207E-09", "module": "A4"}, {"value": "2.89328775996135E-08", "module": "A5"}, {"value": "6.41305327216989E-11", "module": "C1"}, {"value": "1.3999938434862E-09", "module": "C2"}, {"value": "0", "module": "C3"}, {"value": "2.52955296747327E-08", "module": "C4"}, {"value": "-3.79081828398727E-09", "module": "D"}]}}, {"referenceToLCIAMethodDataSet": {"shortDescription": [{"value": "Eutrophication potential aquatic marine (EP-marine)", "lang": "en"}, {"value": "Eutrophierungspotenzial Salzwasser (EP-marine)", "lang": "de"}], "type": "LCIA method data set", "refObjectId": "b5c619fa-def3-11e6-bf01-fe55135034f3", "uri": "../lciamethods/b5c619fa-def3-11e6-bf01-fe55135034f3.xml"}, "other": {"anies": [{"name": "referenceToUnitGroupDataSet", "value": {"shortDescription": [{"value": "kg N eq", "lang": "en"}], "type": "unit group data set", "refObjectId": "d05bb823-ecdf-4686-8c40-bf1d9257859f", "uri": "../unitgroups/d05bb823-ecdf-4686-8c40-bf1d9257859f.xml"}}, {"value": "0.000219881289310719", "module": "A1-A3"}, {"value": "3.07138515658263E-05", "module": "A4"}, {"value": "4.34418207716005E-06", "module": "A5"}, {"value": "1.64860045602368E-06", "module": "C1"}, {"value": "8.885371012181E-06", "module": "C2"}, {"value": "0", "module": "C3"}, {"value": "2.70522724893474E-05", "module": "C4"}, {"value": "-1.07259142025611E-06", "module": "D"}]}}, {"referenceToLCIAMethodDataSet": {"shortDescription": [{"value": "Eutrophication potential terrestrial (EP-terrestrial)", "lang": "en"}, {"value": "Eutrophierungspotenzial Land (EP-terrestrial)", "lang": "de"}], "type": "LCIA method data set", "refObjectId": "b5c614d2-def3-11e6-bf01-fe55135034f3", "uri": "../lciamethods/b5c614d2-def3-11e6-bf01-fe55135034f3.xml"}, "other": {"anies": [{"name": "referenceToUnitGroupDataSet", "value": {"shortDescription": [{"value": "mol N eq", "lang": "en"}], "type": "unit group data set", "refObjectId": "71b4d617-0ec9-4d3f-b65e-e438940c2401", "uri": "../unitgroups/71b4d617-0ec9-4d3f-b65e-e438940c2401.xml"}}, {"value": "0.00228178629300377", "module": "A1-A3"}, {"value": "0.000337484873834702", "module": "A4"}, {"value": "4.95831298332578E-05", "module": "A5"}, {"value": "1.80556515412239E-05", "module": "C1"}, {"value": "9.779920154526E-05", "module": "C2"}, {"value": "0", "module": "C3"}, {"value": "0.000297254634266515", "module": "C4"}, {"value": "-1.1523879108417E-05", "module": "D"}]}}, {"referenceToLCIAMethodDataSet": {"shortDescription": [{"value": "Formation potential of tropospheric ozone photochemical oxidants (POCP)", "lang": "en"}, {"value": "Bildungspotential für troposphärisches Ozon (POCP)", "lang": "de"}], "type": "LCIA method data set", "refObjectId": "b5c610fe-def3-11e6-bf01-fe55135034f3", "uri": "../lciamethods/b5c610fe-def3-11e6-bf01-fe55135034f3.xml"}, "other": {"anies": [{"name": "referenceToUnitGroupDataSet", "value": {"shortDescription": [{"value": "kg NMVOC eq", "lang": "en"}], "type": "unit group data set", "refObjectId": "d27c25f8-fbc1-44c6-b47b-4adbae4199c6", "uri": "../unitgroups/d27c25f8-fbc1-44c6-b47b-4adbae4199c6.xml"}}, {"value": "0.00106257010856927", "module": "A1-A3"}, {"value": "6.19874361907144E-05", "module": "A4"}, {"value": "1.59828073414156E-05", "module": "A5"}, {"value": "4.9473725394444E-06", "module": "C1"}, {"value": "1.77018079201951E-05", "module": "C2"}, {"value": "0", "module": "C3"}, {"value": "8.22124943560373E-05", "module": "C4"}, {"value": "-3.01780340355641E-06", "module": "D"}]}}, {"referenceToLCIAMethodDataSet": {"shortDescription": [{"value": "Abiotic depletion potential for non fossil resources (ADPE)", "lang": "en"}, {"value": "Potenzial für den abiotischen Abbau nicht fossiler Ressourcen (ADPE)", "lang": "de"}], "type": "LCIA method data set", "refObjectId": "b2ad6494-c78d-11e6-9d9d-cec0c932ce01", "uri": "../lciamethods/b2ad6494-c78d-11e6-9d9d-cec0c932ce01.xml"}, "other": {"anies": [{"name": "referenceToUnitGroupDataSet", "value": {"shortDescription": [{"value": "kg Sb eq", "lang": "en"}], "type": "unit group data set", "refObjectId": "54ccd2d9-a32a-4fc2-923d-f2c8c93e89d4", "uri": "../unitgroups/54ccd2d9-a32a-4fc2-923d-f2c8c93e89d4.xml"}}, {"value": "7.98647340832899E-08", "module": "A1-A3"}, {"value": "1.20053813792896E-09", "module": "A4"}, {"value": "8.29955471900874E-10", "module": "A5"}, {"value": "1.4392864839832E-11", "module": "C1"}, {"value": "3.14201696301766E-10", "module": "C2"}, {"value": "0", "module": "C3"}, {"value": "1.52956993412747E-09", "module": "C4"}, {"value": "-4.31812570874023E-10", "module": "D"}]}}, {"referenceToLCIAMethodDataSet": {"shortDescription": [{"value": "Abiotic depletion potential for fossil resources (ADPF)", "lang": "en"}, {"value": "Potenzial für den abiotischen Abbau fossiler Brennstoffe (ADPF)", "lang": "de"}], "type": "LCIA method data set", "refObjectId": "b2ad6110-c78d-11e6-9d9d-cec0c932ce01", "uri": "../lciamethods/b2ad6110-c78d-11e6-9d9d-cec0c932ce01.xml"}, "other": {"anies": [{"name": "referenceToUnitGroupDataSet", "value": {"shortDescription": [{"value": "MJ", "lang": "en"}], "type": "unit group data set", "refObjectId": "93a60a57-a3c8-11da-a746-0800200c9a66", "uri": "../unitgroups/93a60a57-a3c8-11da-a746-0800200c9a66.xml"}}, {"value": "11.7044059764692", "module": "A1-A3"}, {"value": "0.320463007093338", "module": "A4"}, {"value": "0.125111196545931", "module": "A5"}, {"value": "0.00384192771686312", "module": "C1"}, {"value": "0.0838707386709022", "module": "C2"}, {"value": "0", "module": "C3"}, {"value": "0.195496566951586", "module": "C4"}, {"value": "-0.0529178198484462", "module": "D"}]}}, {"referenceToLCIAMethodDataSet": {"shortDescription": [{"value": "Water use (WDP)", "lang": "en"}, {"value": "Wassernutzung (WDP)", "lang": "de"}], "type": "LCIA method data set", "refObjectId": "b2ad66ce-c78d-11e6-9d9d-cec0c932ce01", "uri": "../lciamethods/b2ad66ce-c78d-11e6-9d9d-cec0c932ce01.xml"}, "other": {"anies": [{"name": "referenceToUnitGroupDataSet", "value": {"shortDescription": [{"value": "m^(3) world eq deprived", "lang": "en"}], "type": "unit group data set", "refObjectId": "6ae2df01-888e-46c8-b17d-49fa3869b476", "uri": "../unitgroups/6ae2df01-888e-46c8-b17d-49fa3869b476.xml"}}, {"value": "0.153119241531505", "module": "A1-A3"}, {"value": "6.19484106211873E-05", "module": "A4"}, {"value": "0.00309909350725438", "module": "A5"}, {"value": "7.42679530907097E-07", "module": "C1"}, {"value": "1.62129757359921E-05", "module": "C2"}, {"value": "0", "module": "C3"}, {"value": "0.00163643729662853", "module": "C4"}, {"value": "-0.00029276855852259", "module": "D"}]}}, {"referenceToLCIAMethodDataSet": {"shortDescription": [{"value": "Incidence of disease due to PM emissions (PM)", "lang": "en"}, {"value": "Auftreten von Krankheiten aufgrund von Feinstaubemissionen (PM)", "lang": "de"}], "type": "LCIA method data set", "refObjectId": "b5c602c6-def3-11e6-bf01-fe55135034f3", "uri": "../lciamethods/b5c602c6-def3-11e6-bf01-fe55135034f3.xml"}, "other": {"anies": [{"name": "referenceToUnitGroupDataSet", "value": {"shortDescription": [{"value": "Disease incidence", "lang": "en"}], "type": "unit group data set", "refObjectId": "3883559b-648f-4afc-8ba2-0bd24f3affa3", "uri": "../unitgroups/3883559b-648f-4afc-8ba2-0bd24f3affa3.xml"}}, {"value": "7.36601182780506E-09", "module": "A1-A3"}, {"value": "3.82443821534615E-10", "module": "A4"}, {"value": "1.03614727016379E-10", "module": "A5"}, {"value": "1.93188508789413E-10", "module": "C1"}, {"value": "1.06141722094495E-10", "module": "C2"}, {"value": "0", "module": "C3"}, {"value": "1.30197529852258E-09", "module": "C4"}, {"value": "-3.16815994333158E-11", "module": "D"}]}}, {"referenceToLCIAMethodDataSet": {"shortDescription": [{"value": "Human exposure efficiency relative to U235 (IR)", "lang": "en"}, {"value": "Wirkung durch Exposition des Menschen mit U235 (IR)", "lang": "de"}], "type": "LCIA method data set", "refObjectId": "b5c632be-def3-11e6-bf01-fe55135034f3", "uri": "../lciamethods/b5c632be-def3-11e6-bf01-fe55135034f3.xml"}, "other": {"anies": [{"name": "referenceToUnitGroupDataSet", "value": {"shortDescription": [{"value": "kBq U235 eq", "lang": "en"}], "type": "unit group data set", "refObjectId": "456b05bf-1415-44a9-9993-02452f554c09", "uri": "../unitgroups/456b05bf-1415-44a9-9993-02452f554c09.xml"}}, {"value": "0.0614292227518027", "module": "A1-A3"}, {"value": "7.96214016412766E-05", "module": "A4"}, {"value": "0.000652681538273049", "module": "A5"}, {"value": "9.54555324796085E-07", "module": "C1"}, {"value": "2.08383046462566E-05", "module": "C2"}, {"value": "0", "module": "C3"}, {"value": "0.000242063210897277", "module": "C4"}, {"value": "-0.000621391344493914", "module": "D"}]}}, {"referenceToLCIAMethodDataSet": {"shortDescription": [{"value": "Comparative toxic unit for ecosystems (ETP-fw)", "lang": "en"}, {"value": "Toxizitätsvergleichseinheit für Ökosysteme (ETP-fw)", "lang": "de"}], "type": "LCIA method data set", "refObjectId": "ee1082d1-b0f7-43ca-a1f0-21e2a4a74511", "uri": "../lciamethods/ee1082d1-b0f7-43ca-a1f0-21e2a4a74511.xml"}, "other": {"anies": [{"name": "referenceToUnitGroupDataSet", "value": {"shortDescription": [{"value": "CTUe", "lang": "en"}], "type": "unit group data set", "refObjectId": "aa959ded-f1eb-4efb-9c5c-2d60be36b3e6", "uri": "../unitgroups/aa959ded-f1eb-4efb-9c5c-2d60be36b3e6.xml"}}, {"value": "6.56467548974881", "module": "A1-A3"}, {"value": "0.227954133213166", "module": "A4"}, {"value": "0.0719236142930557", "module": "A5"}, {"value": "0.00273766085571691", "module": "C1"}, {"value": "0.0596616048237011", "module": "C2"}, {"value": "0", "module": "C3"}, {"value": "0.109515161502367", "module": "C4"}, {"value": "-0.0102788948574584", "module": "D"}]}}, {"referenceToLCIAMethodDataSet": {"shortDescription": [{"value": "Comparative toxic unit for humans (carcinogenic) (HTP-c)", "lang": "en"}, {"value": "Toxizitätsvergleichseinheit für Menschen (krebserregend) (HTP-c)", "lang": "de"}], "type": "LCIA method data set", "refObjectId": "2299222a-bbd8-474f-9d4f-4dd1f18aea7c", "uri": "../lciamethods/2299222a-bbd8-474f-9d4f-4dd1f18aea7c.xml"}, "other": {"anies": [{"name": "referenceToUnitGroupDataSet", "value": {"shortDescription": [{"value": "CTUh", "lang": "en"}], "type": "unit group data set", "refObjectId": "d4c9523e-2d7e-49fd-8469-998f547d3a70", "uri": "../unitgroups/d4c9523e-2d7e-49fd-8469-998f547d3a70.xml"}}, {"value": "1.48032475805006E-10", "module": "A1-A3"}, {"value": "4.24683806509521E-12", "module": "A4"}, {"value": "1.75890287840393E-12", "module": "A5"}, {"value": "5.08864220100882E-14", "module": "C1"}, {"value": "1.11145844126781E-12", "module": "C2"}, {"value": "0", "module": "C3"}, {"value": "1.67140201023442E-11", "module": "C4"}, {"value": "-5.18484276208461E-13", "module": "D"}]}}, {"referenceToLCIAMethodDataSet": {"shortDescription": [{"value": "Comparative toxic unit for humans (noncarcinogenic) (HTP-nc)", "lang": "en"}, {"value": "Toxizitätsvergleichseinheit für Menschen (nicht krebserregend) (HTP-nc)", "lang": "de"}], "type": "LCIA method data set", "refObjectId": "3af763a5-b7a1-48c9-9cee-1f223481fcef", "uri": "../lciamethods/3af763a5-b7a1-48c9-9cee-1f223481fcef.xml"}, "other": {"anies": [{"name": "referenceToUnitGroupDataSet", "value": {"shortDescription": [{"value": "CTUh", "lang": "en"}], "type": "unit group data set", "refObjectId": "d4c9523e-2d7e-49fd-8469-998f547d3a70", "uri": "../unitgroups/d4c9523e-2d7e-49fd-8469-998f547d3a70.xml"}}, {"value": "7.93941293013164E-09", "module": "A1-A3"}, {"value": "2.0805325846098E-10", "module": "A4"}, {"value": "1.14000128772375E-10", "module": "A5"}, {"value": "3.52087228510558E-12", "module": "C1"}, {"value": "5.50997136711837E-11", "module": "C2"}, {"value": "0", "module": "C3"}, {"value": "1.85088606482084E-09", "module": "C4"}, {"value": "-2.00539809913155E-11", "module": "D"}]}}, {"referenceToLCIAMethodDataSet": {"shortDescription": [{"value": "Soil quality index (SQP)", "lang": "en"}, {"value": "Bodenqualitätsindex (SQP)", "lang": "de"}], "type": "LCIA method data set", "refObjectId": "b2ad6890-c78d-11e6-9d9d-cec0c932ce01", "uri": "../lciamethods/b2ad6890-c78d-11e6-9d9d-cec0c932ce01.xml"}, "other": {"anies": [{"name": "referenceToUnitGroupDataSet", "value": {"shortDescription": [{"value": "SQP", "lang": "en"}], "type": "unit group data set", "refObjectId": "f130951c-e67f-4f7f-8dd4-665de3974e18", "uri": "../unitgroups/f130951c-e67f-4f7f-8dd4-665de3974e18.xml"}}, {"value": "0.680562995555687", "module": "A1-A3"}, {"value": "0.00190258576520719", "module": "A4"}, {"value": "0.00800977058706664", "module": "A5"}, {"value": "2.28094875953334E-05", "module": "C1"}, {"value": "0.000497939762096142", "module": "C2"}, {"value": "0", "module": "C3"}, {"value": "0.040670203680629", "module": "C4"}, {"value": "-0.00832165822760573", "module": "D"}]}}]}, "otherAttributes": {"{http://www.indata.network/EPD/2019}epd-version": "1.2"}, "version": "1.1", "locations": "../ILCDLocations.xml"}