{"processInformation": {"dataSetInformation": {"UUID": "d8f28c30-9229-44c0-b4ae-5a425c542d89", "name": {"baseName": [{"value": "Medium Density Fibreboard (MDF)", "lang": "en"}, {"value": "Medium Density Fibreboard (MDF)", "lang": "de"}], "functionalUnitFlowProperties": [{"lang": "en"}]}, "classificationInformation": {"classification": [{"class": [{"value": "Holz", "level": 0, "classId": "3"}, {"value": "Holzwerkstoffe", "level": 1, "classId": "3.2"}, {"value": "Holzfaserplatten", "level": 2, "classId": "3.2.07"}], "name": "OEKOBAU.DAT"}, {"class": [{"value": "02 Building products", "level": 0}, {"value": "Wood based panels", "level": 1}, {"value": "Wood-based panels", "level": 2}], "name": "IBUCategories"}]}, "generalComment": [{"value": "MDF (Medium Density Fibreboard) is engineered wood products that consist of panels made from a combination of wood fibres and resin. They are applicable particularly in furniture such as doors, construction such as mouldings and indoor products. It is especially suitable for further finishing (routing, milling, lacquering, laminating and foiling) and a good substitute for solid wood.\nThe Kronobuild® product line includes, as well as standard MDF, boards with specialist application properties  moisture resistant MR MDF, Light MDF and Ultra Light MDF, Flame Retardant MDF, Deep Router MDF.", "lang": "en"}, {"value": "MDF (Medium Density Fibreboard) sind Holzwerkstoffe, die aus einer Kombination aus Holzfasern und Harz bestehen. Sie werden vor allem für Möbel wie Türen, Konstruktionen wie Leisten und Produkte für den Innenbereich verwendet. Sie eignen sich besonders für die Weiterverarbeitung (Fräsen, Lackieren, Laminieren und Folieren) und sind ein guter Ersatz für Massivholz. Die Kronobuild®-Produktlinie umfasst neben Standard-MDF-Platten auch Platten mit speziellen Anwendungseigenschaften - feuchtigkeitsbeständiges MR MDF, Light MDF und Ultra Light MDF, flammhemmendes MDF, Deep Router MDF.", "lang": "de"}]}, "quantitativeReference": {"referenceToReferenceFlow": [0]}, "time": {"referenceYear": 2023, "dataSetValidUntil": 2028, "other": {"anies": [{"name": "publicationDateOfEPD", "value": 1689033600000}]}}, "geography": {"locationOfOperationSupplyOrProduction": {"location": "LU"}}, "technology": {"technologyDescriptionAndIncludedProcesses": [{"value": "First, the wood logs go through a hacker. The obtained shavings are refined and dried. The materials are then blended with the resin and pressed to obtain panels. A finishing process is finally done to cut and pack the products. \nTechnical data: \nTechnical product groups covered in this EPD are MDF Light, Standard MDF, Moisture Resistant MDF, Deep Router MDF, Flame Retardant, Ultra Light MDF.\n\nTechnical specification accounts for thicknesses of boards within the range of 5,5 - 38mm. \nDeclared unit: \nThis declaration applies to 1 m3 of Kronospan MDF panel, with a declared unit weight of 716.7 kg/m3.", "lang": "en"}, {"value": "Zuerst werden die Holzstämme durch einen Hacker geführt. Die gewonnenen Späne werden veredelt und getrocknet. Die Materialien werden dann mit dem Harz vermischt und zu Platten gepresst. Zum Schluss werden die Produkte geschnitten und verpackt. \nTechnische Daten: \nDie technischen Produktgruppen, die in dieser EPD behandelt werden, sind MDF Light, Standard MDF, feuchtigkeitsbeständige MDF, Deep Router MDF, flammhemmende MDF, Ultra Light MDF. Die technische Spezifikation berücksichtigt Plattenstärken im Bereich von 5,5 - 38 mm. \nDeklarierte Einheit: \nDiese Erklärung gilt für 1 m3 Kronospan MDF-Platte mit einem deklarierten Stückgewicht von 716,7 kg/m3.", "lang": "de"}], "technologicalApplicability": [{"value": "Due to their homogeneous structure, MDF boards can be milled three-dimensionally and then painted, foil wrapped or faced with a paper decor in a membrane press.\nThe main applications of MDF include interior design, furniture components, decorative features, cladding, partitions, areas that require protection from moisture, skirting boards / architrave and window boards / sills.", "lang": "en"}, {"value": "Aufgrund ihrer homogenen Struktur können MDF-Platten dreidimensional gefräst und anschließend in einer Membranpresse lackiert, mit Folie ummantelt oder mit einem Papierdekor versehen werden. Zu den Hauptanwendungen von MDF gehören der Innenausbau, Möbelkomponenten, dekorative Elemente, Verkleidungen, Trennwände, Bereiche, die vor Feuchtigkeit geschützt werden müssen, Sockelleisten/Architrave und Fensterbänke.", "lang": "de"}]}}, "modellingAndValidation": {"LCIMethodAndAllocation": {"typeOfDataSet": "EPD", "referenceToLCAMethodDetails": [{"shortDescription": [{"value": "Wood-based panels.pdf", "lang": "en"}], "type": "source data set", "refObjectId": "3500cbb5-6ff2-45af-950f-7bff6cfbd8bd"}], "other": {"anies": [{"name": "subType", "value": "specific dataset"}]}}, "dataSourcesTreatmentAndRepresentativeness": {"referenceToDataSource": [{"shortDescription": [{"value": "ecoinvent database (all versions)", "lang": "en"}], "type": "source data set", "refObjectId": "b497a91f-e14b-4b69-8f28-f50eb1576766"}, {"shortDescription": [{"value": "ecoinvent 3.8 database", "lang": "en"}], "type": "source data set", "refObjectId": "0f4c65c0-6210-450f-b886-82bf8dd5ace9"}], "useAdviceForDataSet": [{"value": "Scope: \nThis document applies to Kronospan MDF, which is composed of wood shavings, mixed with a resin (melamine urea formaldehyde – MUF). \nThe declared unit weight is 716.7 kg/m3. LCA data were compiled using foreground data collected based on billing documents and material balances for the period between October 2020 and March 2022. The declaration holder is responsible for the underlying data and its verification. \nSystem boundary: \nType of EPD: Cradle-to-grave (with options)\nThe system boundaries of the EPD follow the modular construction system as described by EN 15804.\n\nThe LCA considers the following modules:\n\nA1-A3: Manufacturing of pre-products, packaging, ancillary materials, transport to the factory and production, with the associated energy supply and waste handling\nA4: Transport to the construction site\nA5: Installation into the building including disposal of packaging\nC1: Deconstruction (screws disposal and electricity from the screwdriver)· C2: Transport to disposal sites\nC3: Final product waste disposal for reuse, recycling and energy recovery\nC4: Waste disposal, namely incineration and landfill\nD: Potential for reuse, recovery and/or recycling including benefits for product incineration from module C4", "lang": "en"}, {"value": "Gültigkeitsbereich: \nDieses Dokument gilt für Kronospan MDF, das aus Holzspänen besteht, die mit einem Harz (Melamin-Harnstoff-Formaldehyd - MUF) gemischt sind. \nDas angegebene Stückgewicht beträgt 716,7 kg/m3. Die Ökobilanzdaten wurden anhand von Vordergrunddaten zusammengestellt, die auf der Grundlage von Rechnungsunterlagen und Materialbilanzen für den Zeitraum zwischen Oktober 2020 und März 2022 erhoben wurden. Der Deklarationsinhaber ist für die zugrunde liegenden Daten und deren Überprüfung verantwortlich. \nSystemgrenze: \nArt der EPD: Cradle-to-Grave (mit Optionen) Die Systemgrenzen der EPD folgen dem modularen Bausystem, wie es in EN 15804 beschrieben ist.\n\nDie Ökobilanz berücksichtigt die folgenden Module: A1-A3: Herstellung von Vorprodukten, Verpackung, Hilfsstoffen, Transport zum Werk und zur Produktion, mit der damit verbundenen Energieversorgung und Abfallbehandlung A4: Transport zur Baustelle A5: Einbau in das Gebäude einschließlich Entsorgung der Verpackung C1: Rückbau (Schraubenentsorgung und Strom aus dem Schraubenzieher)- C2: Transport zu den Entsorgungsstellen C3: Entsorgung des Endprodukts zur Wiederverwendung, zum Recycling und zur Energierückgewinnung C4: Abfallentsorgung, nämlich Verbrennung und Deponierung D: Potenzial für Wiederverwendung, Rückgewinnung und/oder Recycling einschließlich der Vorteile der Produktverbrennung aus Modul C4", "lang": "de"}], "other": {"anies": [{"name": "referenceToOriginalEPD", "value": {"shortDescription": {"value": "Medium Density Fibreboard (MDF).pdf", "defaultValue": "Medium Density Fibreboard (MDF).pdf", "lstrings": [{"lang": "en", "value": "Medium Density Fibreboard (MDF).pdf"}]}, "type": "source data set", "uuid": {"uuid": "2406da41-58b3-4272-a091-2a4843dcf3fe"}, "refObjectId": "2406da41-58b3-4272-a091-2a4843dcf3fe", "resourceURLs": ["https://oekobaudat.de/OEKOBAU.DAT/resource/sources/2406da41-58b3-4272-a091-2a4843dcf3fe/Medium_Density_Fibreboard_MDF__16704.pdf?version=00.01.000"]}}]}}, "validation": {"review": [{"referenceToNameOfReviewerAndInstitution": [{"shortDescription": [{"value": "Institut Bauen und Umwelt e. V.", "lang": "en"}], "type": "contact data set", "refObjectId": "d111dbec-b024-4be5-86c5-752d6eb2cf95", "uri": "../contacts/d111dbec-b024-4be5-86c5-752d6eb2cf95.xml"}], "type": "Accredited third party review"}]}, "complianceDeclarations": {"compliance": [{"referenceToComplianceSystem": {"shortDescription": [{"value": "DIN EN 15804+A2", "lang": "en"}], "type": "source data set", "refObjectId": "c0016b33-8cf7-415c-ac6e-deba0d21440d", "uri": "../sources/c0016b33-8cf7-415c-ac6e-deba0d21440d.xml"}}, {"referenceToComplianceSystem": {"shortDescription": [{"value": "ISO 14025", "lang": "en"}], "type": "source data set", "refObjectId": "4f2eb655-6e44-4874-a95a-e28f5442cd4d", "uri": "../sources/4f2eb655-6e44-4874-a95a-e28f5442cd4d.xml"}}]}}, "administrativeInformation": {"commissionerAndGoal": {"referenceToCommissioner": [{"shortDescription": [{"value": "Kronospan Luxembourg S.A.", "lang": "en"}], "type": "contact data set", "refObjectId": "b0fc2464-4d12-49c7-a343-f7fdb7963fcd", "uri": "../contacts/b0fc2464-4d12-49c7-a343-f7fdb7963fcd.xml"}]}, "dataGenerator": {"referenceToPersonOrEntityGeneratingTheDataSet": [{"shortDescription": [{"value": "Luxembourg Institute of Science and Technology (LIST)", "lang": "en"}], "type": "contact data set", "refObjectId": "3dc32f52-ebeb-41a9-9c79-c39364b358a5", "uri": "../contacts/3dc32f52-ebeb-41a9-9c79-c39364b358a5.xml"}]}, "dataEntryBy": {"timeStamp": 1689033600000, "referenceToDataSetFormat": [{"shortDescription": [{"value": "ILCD Format", "lang": "en"}], "type": "source data set", "refObjectId": "a97a0155-0234-4b87-b4ce-a45da52f2a40", "uri": "../sources/a97a0155-0234-4b87-b4ce-a45da52f2a40.xml"}, {"shortDescription": [{"value": "EPD-Datenformaterweiterungen v1.2", "lang": "de"}, {"value": "EPD Data Format Extensions v1.2", "lang": "en"}], "type": "source data set", "refObjectId": "a29449fd-aa2f-4de8-b5d7-4b06b43c6fde", "uri": "../sources/a29449fd-aa2f-4de8-b5d7-4b06b43c6fde.xml"}]}, "publicationAndOwnership": {"dataSetVersion": "00.03.000", "referenceToRegistrationAuthority": {"shortDescription": [{"value": "Institut Bauen und Umwelt e. V.", "lang": "en"}], "type": "contact data set", "refObjectId": "d111dbec-b024-4be5-86c5-752d6eb2cf95", "uri": "../contacts/d111dbec-b024-4be5-86c5-752d6eb2cf95.xml"}, "registrationNumber": "EPD-KRO-20230159-CBA1-EN", "referenceToOwnershipOfDataSet": {"shortDescription": [{"value": "Kronospan Luxembourg S.A.", "lang": "en"}], "type": "contact data set", "refObjectId": "b0fc2464-4d12-49c7-a343-f7fdb7963fcd", "uri": "../contacts/b0fc2464-4d12-49c7-a343-f7fdb7963fcd.xml"}, "copyright": true, "licenseType": "Free of charge for all users and uses", "accessRestrictions": [{"value": "None", "lang": "en"}], "other": {"anies": [{"name": "referenceToPublisher", "value": {"shortDescription": [{"value": "Institut Bauen und Umwelt e. V.", "lang": "en"}], "type": "contact data set", "refObjectId": "d111dbec-b024-4be5-86c5-752d6eb2cf95", "uri": "../contacts/d111dbec-b024-4be5-86c5-752d6eb2cf95.xml"}}]}}}, "exchanges": {"exchange": [{"dataSetInternalID": 0, "referenceToFlowDataSet": {"shortDescription": [{"value": "Kronospan MDF panel (Kronospan MDF panel)", "lang": "en"}], "type": "flow data set", "refObjectId": "38527ded-ec38-7718-7857-f53f401cfc16", "uri": "../flows/38527ded-ec38-7718-7857-f53f401cfc16.xml"}, "meanAmount": 1.0, "referencesToDataSource": {}, "referenceFlow": true, "resolvedFlowVersion": "00.03.000", "resultingflowAmount": 1.0, "flowProperties": [{"name": [{"lang": "en", "value": "Volume"}, {"lang": "de", "value": "Volumen"}], "uuid": "93a60a56-a3c8-22da-a746-0800200c9a66", "referenceFlowProperty": true, "meanValue": 1.0, "referenceUnit": "m3", "unitGroupUUID": "cd950537-0a98-4044-9ba7-9f9a68d0a504"}], "materialProperties": [{"name": "layer thickness", "value": "0.014", "unit": "m", "unitDescription": "meters"}, {"name": "gross density", "value": "716.7", "unit": "kg/m^3", "unitDescription": "kilograms per cubic metre"}], "typeOfFlow": "Product flow", "classification": {"classHierarchy": "Holz / Holzwerkstoffe / Holzfaserplatten", "name": "OEKOBAU.DAT"}}, {"dataSetInternalID": 1, "referenceToFlowDataSet": {"shortDescription": [{"value": "Renewable primary energy as energy carrier (PERE)", "lang": "en"}, {"value": "Erneuerbare Primärenergie als Energieträger (PERE)", "lang": "de"}], "type": "flow data set", "refObjectId": "20f32be5-0398-4288-9b6d-accddd195317", "uri": "../flows/20f32be5-0398-4288-9b6d-accddd195317.xml"}, "exchange direction": "INPUT", "other": {"anies": [{"name": "referenceToUnitGroupDataSet", "value": {"shortDescription": [{"value": "MJ", "lang": "en"}], "type": "unit group data set", "refObjectId": "93a60a57-a3c8-11da-a746-0800200c9a66", "uri": "../unitgroups/93a60a57-a3c8-11da-a746-0800200c9a66.xml"}}, {"value": "153.163184450133", "module": "A1-A3"}, {"value": "5.29785343976546", "module": "A4"}, {"value": "3.95899948482029", "module": "A5"}, {"value": "0.124916299458935", "module": "C1"}, {"value": "1.26912700692624", "module": "C2"}, {"value": "0", "module": "C3"}, {"value": "8320", "module": "C4"}, {"value": "0", "module": "D"}]}, "resolvedFlowVersion": "38.00.000", "flowProperties": [], "typeOfFlow": "Other flow", "classification": {"classHierarchy": "Quantities", "name": "GaBiCategories"}}, {"dataSetInternalID": 2, "referenceToFlowDataSet": {"shortDescription": [{"value": "Renewable primary energy resources as material utilization (PERM)", "lang": "en"}, {"value": "Erneuerbare Primärenergie zur stofflichen Nutzung (PERM)", "lang": "de"}], "type": "flow data set", "refObjectId": "fb3ec0de-548d-4508-aea5-00b73bf6f702", "uri": "../flows/fb3ec0de-548d-4508-aea5-00b73bf6f702.xml"}, "exchange direction": "INPUT", "other": {"anies": [{"name": "referenceToUnitGroupDataSet", "value": {"shortDescription": [{"value": "MJ", "lang": "en"}], "type": "unit group data set", "refObjectId": "93a60a57-a3c8-11da-a746-0800200c9a66", "uri": "../unitgroups/93a60a57-a3c8-11da-a746-0800200c9a66.xml"}}, {"value": "16681.9243831701", "module": "A1-A3"}, {"value": "0", "module": "A4"}, {"value": "0", "module": "A5"}, {"value": "0", "module": "C1"}, {"value": "0", "module": "C2"}, {"value": "0", "module": "C3"}, {"value": "-8320", "module": "C4"}, {"value": "0", "module": "D"}]}, "resolvedFlowVersion": "38.00.000", "flowProperties": [], "typeOfFlow": "Other flow", "classification": {"classHierarchy": "Quantities", "name": "GaBiCategories"}}, {"dataSetInternalID": 3, "referenceToFlowDataSet": {"shortDescription": [{"value": "Total use of renewable primary energy resources (PERT)", "lang": "en"}, {"value": "Total erneuerbare Primärenergie (PERT)", "lang": "de"}], "type": "flow data set", "refObjectId": "53f97275-fa8a-4cdd-9024-65936002acd0", "uri": "../flows/53f97275-fa8a-4cdd-9024-65936002acd0.xml"}, "exchange direction": "INPUT", "other": {"anies": [{"name": "referenceToUnitGroupDataSet", "value": {"shortDescription": [{"value": "MJ", "lang": "en"}], "type": "unit group data set", "refObjectId": "93a60a57-a3c8-11da-a746-0800200c9a66", "uri": "../unitgroups/93a60a57-a3c8-11da-a746-0800200c9a66.xml"}}, {"value": "16835.0875676203", "module": "A1-A3"}, {"value": "5.29785343976546", "module": "A4"}, {"value": "3.95899948482029", "module": "A5"}, {"value": "0.124916299458935", "module": "C1"}, {"value": "1.26912700692624", "module": "C2"}, {"value": "0", "module": "C3"}, {"value": "0", "module": "C4"}, {"value": "0", "module": "D"}]}, "resolvedFlowVersion": "38.00.000", "flowProperties": [], "typeOfFlow": "Other flow", "classification": {"classHierarchy": "Quantities / Environmental quantities / EPD EN 15804 / LCI indicators", "name": "GaBiCategories"}}, {"dataSetInternalID": 4, "referenceToFlowDataSet": {"shortDescription": [{"value": "Non renewable primary energy as energy carrier (PENRE)", "lang": "en"}, {"value": "Nicht-erneuerbare Primärenergie als Energieträger (PENRE)", "lang": "de"}], "type": "flow data set", "refObjectId": "ac857178-2b45-46ec-892a-a9a4332f0372", "uri": "../flows/ac857178-2b45-46ec-892a-a9a4332f0372.xml"}, "exchange direction": "INPUT", "other": {"anies": [{"name": "referenceToUnitGroupDataSet", "value": {"shortDescription": [{"value": "MJ", "lang": "en"}], "type": "unit group data set", "refObjectId": "93a60a57-a3c8-11da-a746-0800200c9a66", "uri": "../unitgroups/93a60a57-a3c8-11da-a746-0800200c9a66.xml"}}, {"value": "6066.88029406866", "module": "A1-A3"}, {"value": "441.975591968656", "module": "A4"}, {"value": "57.1833573282983", "module": "A5"}, {"value": "0.636515809543196", "module": "C1"}, {"value": "95.5975316156508", "module": "C2"}, {"value": "0", "module": "C3"}, {"value": "89.4849176698622", "module": "C4"}, {"value": "-3855.79212888688", "module": "D"}]}, "resolvedFlowVersion": "38.00.000", "flowProperties": [], "typeOfFlow": "Other flow", "classification": {"classHierarchy": "Quantities", "name": "GaBiCategories"}}, {"dataSetInternalID": 5, "referenceToFlowDataSet": {"shortDescription": [{"value": "Non renewable primary energy as material utilization (PENRM)", "lang": "en"}, {"value": "Nicht-erneuerbare Primärenergie zur stofflichen Nutzung (PENRM)", "lang": "de"}], "type": "flow data set", "refObjectId": "1421caa0-679d-4bf4-b282-0eb850ccae27", "uri": "../flows/1421caa0-679d-4bf4-b282-0eb850ccae27.xml"}, "exchange direction": "INPUT", "other": {"anies": [{"name": "referenceToUnitGroupDataSet", "value": {"shortDescription": [{"value": "MJ", "lang": "en"}], "type": "unit group data set", "refObjectId": "93a60a57-a3c8-11da-a746-0800200c9a66", "uri": "../unitgroups/93a60a57-a3c8-11da-a746-0800200c9a66.xml"}}, {"value": "0", "module": "A1-A3"}, {"value": "0", "module": "A4"}, {"value": "0", "module": "A5"}, {"value": "0", "module": "C1"}, {"value": "0", "module": "C2"}, {"value": "0", "module": "C3"}, {"value": "0", "module": "C4"}, {"value": "0", "module": "D"}]}, "resolvedFlowVersion": "38.00.000", "flowProperties": [], "typeOfFlow": "Other flow", "classification": {"classHierarchy": "Quantities", "name": "GaBiCategories"}}, {"dataSetInternalID": 6, "referenceToFlowDataSet": {"shortDescription": [{"value": "Total use of non renewable primary energy resources (PENRT)", "lang": "en"}, {"value": "Total nicht erneuerbare Primärenergie (PENRT)", "lang": "de"}], "type": "flow data set", "refObjectId": "06159210-646b-4c8d-8583-da9b3b95a6c1", "uri": "../flows/06159210-646b-4c8d-8583-da9b3b95a6c1.xml"}, "exchange direction": "INPUT", "other": {"anies": [{"name": "referenceToUnitGroupDataSet", "value": {"shortDescription": [{"value": "MJ", "lang": "en"}], "type": "unit group data set", "refObjectId": "93a60a57-a3c8-11da-a746-0800200c9a66", "uri": "../unitgroups/93a60a57-a3c8-11da-a746-0800200c9a66.xml"}}, {"value": "6066.88029406866", "module": "A1-A3"}, {"value": "441.975591968656", "module": "A4"}, {"value": "57.1833573282983", "module": "A5"}, {"value": "0.636515809543196", "module": "C1"}, {"value": "95.5975316156508", "module": "C2"}, {"value": "0", "module": "C3"}, {"value": "89.4849176698622", "module": "C4"}, {"value": "-3855.79212888688", "module": "D"}]}, "resolvedFlowVersion": "38.00.000", "flowProperties": [], "typeOfFlow": "Other flow", "classification": {"classHierarchy": "Quantities / Environmental quantities / EPD EN 15804 / LCI indicators", "name": "GaBiCategories"}}, {"dataSetInternalID": 7, "referenceToFlowDataSet": {"shortDescription": [{"value": "Use of secondary material (SM)", "lang": "en"}, {"value": "Einsatz von Sekundärstoffen (SM)", "lang": "de"}], "type": "flow data set", "refObjectId": "c6a1f35f-2d09-4f54-8dfb-97e502e1ce92", "uri": "../flows/c6a1f35f-2d09-4f54-8dfb-97e502e1ce92.xml"}, "exchange direction": "INPUT", "other": {"anies": [{"name": "referenceToUnitGroupDataSet", "value": {"shortDescription": [{"value": "kg", "lang": "en"}], "type": "unit group data set", "refObjectId": "ad38d542-3fe9-439d-9b95-2f5f7752acaf", "uri": "../unitgroups/ad38d542-3fe9-439d-9b95-2f5f7752acaf.xml"}}, {"value": "0", "module": "A1-A3"}, {"value": "0", "module": "A4"}, {"value": "0", "module": "A5"}, {"value": "0", "module": "C1"}, {"value": "0", "module": "C2"}, {"value": "0", "module": "C3"}, {"value": "0", "module": "C4"}, {"value": "0", "module": "D"}]}, "resolvedFlowVersion": "38.00.000", "flowProperties": [], "typeOfFlow": "Other flow", "classification": {"classHierarchy": "Quantities / Environmental quantities / EPD EN 15804 / LCI indicators", "name": "GaBiCategories"}}, {"dataSetInternalID": 8, "referenceToFlowDataSet": {"shortDescription": [{"value": "Use of renewable secondary fuels (RSF)", "lang": "en"}, {"value": "Erneuerbare Sekundärbrennstoffe (RSF)", "lang": "de"}], "type": "flow data set", "refObjectId": "64333088-a55f-4aa2-9a31-c10b07816787", "uri": "../flows/64333088-a55f-4aa2-9a31-c10b07816787.xml"}, "exchange direction": "INPUT", "other": {"anies": [{"name": "referenceToUnitGroupDataSet", "value": {"shortDescription": [{"value": "MJ", "lang": "en"}], "type": "unit group data set", "refObjectId": "93a60a57-a3c8-11da-a746-0800200c9a66", "uri": "../unitgroups/93a60a57-a3c8-11da-a746-0800200c9a66.xml"}}, {"value": "6866.8992", "module": "A1-A3"}, {"value": "0", "module": "A4"}, {"value": "0", "module": "A5"}, {"value": "0", "module": "C1"}, {"value": "0", "module": "C2"}, {"value": "0", "module": "C3"}, {"value": "0", "module": "C4"}, {"value": "8320", "module": "D"}]}, "resolvedFlowVersion": "38.00.000", "flowProperties": [], "typeOfFlow": "Other flow", "classification": {"classHierarchy": "Quantities / Environmental quantities / EPD EN 15804 / LCI indicators", "name": "GaBiCategories"}}, {"dataSetInternalID": 9, "referenceToFlowDataSet": {"shortDescription": [{"value": "Use of non renewable secondary fuels (NRSF)", "lang": "en"}, {"value": "Nicht erneuerbare Sekundärbrennstoffe (NRSF)", "lang": "de"}], "type": "flow data set", "refObjectId": "89def144-d39a-4287-b86f-efde453ddcb2", "uri": "../flows/89def144-d39a-4287-b86f-efde453ddcb2.xml"}, "exchange direction": "INPUT", "other": {"anies": [{"name": "referenceToUnitGroupDataSet", "value": {"shortDescription": [{"value": "MJ", "lang": "en"}], "type": "unit group data set", "refObjectId": "93a60a57-a3c8-11da-a746-0800200c9a66", "uri": "../unitgroups/93a60a57-a3c8-11da-a746-0800200c9a66.xml"}}, {"value": "0", "module": "A1-A3"}, {"value": "0", "module": "A4"}, {"value": "0", "module": "A5"}, {"value": "0", "module": "C1"}, {"value": "0", "module": "C2"}, {"value": "0", "module": "C3"}, {"value": "0", "module": "C4"}, {"value": "0", "module": "D"}]}, "resolvedFlowVersion": "38.00.000", "flowProperties": [], "typeOfFlow": "Other flow", "classification": {"classHierarchy": "Quantities / Environmental quantities / EPD EN 15804 / LCI indicators", "name": "GaBiCategories"}}, {"dataSetInternalID": 10, "referenceToFlowDataSet": {"shortDescription": [{"value": "Use of net fresh water (FW)", "lang": "en"}, {"value": "Einsatz von Süßwasserressourcen (FW)", "lang": "de"}], "type": "flow data set", "refObjectId": "3cf952c8-f3a4-461d-8c96-96456ca62246", "uri": "../flows/3cf952c8-f3a4-461d-8c96-96456ca62246.xml"}, "exchange direction": "INPUT", "other": {"anies": [{"name": "referenceToUnitGroupDataSet", "value": {"shortDescription": [{"value": "m^3", "lang": "en"}], "type": "unit group data set", "refObjectId": "cd950537-0a98-4044-9ba7-9f9a68d0a504", "uri": "../unitgroups/cd950537-0a98-4044-9ba7-9f9a68d0a504.xml"}}, {"value": "13.2384787935915", "module": "A1-A3"}, {"value": "0.206706229930898", "module": "A4"}, {"value": "0.106634938844861", "module": "A5"}, {"value": "0.0100915828009003", "module": "C1"}, {"value": "0.0555543448516101", "module": "C2"}, {"value": "0", "module": "C3"}, {"value": "0.367297000974315", "module": "C4"}, {"value": "-0.197494888662774", "module": "D"}]}, "resolvedFlowVersion": "38.00.000", "flowProperties": [], "typeOfFlow": "Other flow", "classification": {"classHierarchy": "Quantities / Environmental quantities / EPD EN 15804 / LCI indicators", "name": "GaBiCategories"}}, {"dataSetInternalID": 11, "referenceToFlowDataSet": {"shortDescription": [{"value": "Hazardous waste disposed (HWD)", "lang": "en"}, {"value": "Gefährlicher Abfall zur Deponie (HWD)", "lang": "de"}], "type": "flow data set", "refObjectId": "430f9e0f-59b2-46a0-8e0d-55e0e84948fc", "uri": "../flows/430f9e0f-59b2-46a0-8e0d-55e0e84948fc.xml"}, "exchange direction": "OUTPUT", "other": {"anies": [{"name": "referenceToUnitGroupDataSet", "value": {"shortDescription": [{"value": "kg", "lang": "en"}], "type": "unit group data set", "refObjectId": "ad38d542-3fe9-439d-9b95-2f5f7752acaf", "uri": "../unitgroups/ad38d542-3fe9-439d-9b95-2f5f7752acaf.xml"}}, {"value": "0.00833639796672856", "module": "A1-A3"}, {"value": "0.00100736556171901", "module": "A4"}, {"value": "0.000255907368920389", "module": "A5"}, {"value": "4.61572641755167E-07", "module": "C1"}, {"value": "0.000235182893074706", "module": "C2"}, {"value": "0", "module": "C3"}, {"value": "0.000194397623224593", "module": "C4"}, {"value": "-0.00466250729196911", "module": "D"}]}, "resolvedFlowVersion": "38.00.000", "flowProperties": [], "typeOfFlow": "Other flow", "classification": {"classHierarchy": "Quantities / Environmental quantities / EPD EN 15804 / LCI indicators", "name": "GaBiCategories"}}, {"dataSetInternalID": 12, "referenceToFlowDataSet": {"shortDescription": [{"value": "Non hazardous waste disposed (NHWD)", "lang": "en"}, {"value": "Entsorgter nicht gefährlicher Abfall (NHWD)", "lang": "de"}], "type": "flow data set", "refObjectId": "b29ef66b-e286-4afa-949f-62f1a7b4d7fa", "uri": "../flows/b29ef66b-e286-4afa-949f-62f1a7b4d7fa.xml"}, "exchange direction": "OUTPUT", "other": {"anies": [{"name": "referenceToUnitGroupDataSet", "value": {"shortDescription": [{"value": "kg", "lang": "en"}], "type": "unit group data set", "refObjectId": "ad38d542-3fe9-439d-9b95-2f5f7752acaf", "uri": "../unitgroups/ad38d542-3fe9-439d-9b95-2f5f7752acaf.xml"}}, {"value": "53.28105481258", "module": "A1-A3"}, {"value": "38.9465491620271", "module": "A4"}, {"value": "16.9434094876969", "module": "A5"}, {"value": "0.00211904371996323", "module": "C1"}, {"value": "4.63095588401485", "module": "C2"}, {"value": "0", "module": "C3"}, {"value": "125.92551568103", "module": "C4"}, {"value": "-1.90039248315473", "module": "D"}]}, "resolvedFlowVersion": "38.00.000", "flowProperties": [], "typeOfFlow": "Other flow", "classification": {"classHierarchy": "Quantities / Environmental quantities / EPD EN 15804 / LCI indicators", "name": "GaBiCategories"}}, {"dataSetInternalID": 13, "referenceToFlowDataSet": {"shortDescription": [{"value": "Radioactive waste disposed (RWD)", "lang": "en"}, {"value": "Entsorgter radioaktiver Abfall (RWD)", "lang": "de"}], "type": "flow data set", "refObjectId": "3449546e-52ad-4b39-b809-9fb77cea8ff6", "uri": "../flows/3449546e-52ad-4b39-b809-9fb77cea8ff6.xml"}, "exchange direction": "OUTPUT", "other": {"anies": [{"name": "referenceToUnitGroupDataSet", "value": {"shortDescription": [{"value": "kg", "lang": "en"}], "type": "unit group data set", "refObjectId": "ad38d542-3fe9-439d-9b95-2f5f7752acaf", "uri": "../unitgroups/ad38d542-3fe9-439d-9b95-2f5f7752acaf.xml"}}, {"value": "0.010062575135907", "module": "A1-A3"}, {"value": "0.00281821121050295", "module": "A4"}, {"value": "0.000171645654326844", "module": "A5"}, {"value": "4.46294672126117E-06", "module": "C1"}, {"value": "0.000608954780294686", "module": "C2"}, {"value": "0", "module": "C3"}, {"value": "0.00030737979835785", "module": "C4"}, {"value": "-0.000394792147962968", "module": "D"}]}, "resolvedFlowVersion": "38.00.000", "flowProperties": [], "typeOfFlow": "Other flow", "classification": {"classHierarchy": "Quantities / Environmental quantities / EPD EN 15804 / LCI indicators", "name": "GaBiCategories"}}, {"dataSetInternalID": 14, "referenceToFlowDataSet": {"shortDescription": [{"value": "Components for re-use (CRU)", "lang": "en"}, {"value": "Komponenten für die Wiederverwendung (CRU)", "lang": "de"}], "type": "flow data set", "refObjectId": "a2b32f97-3fc7-4af2-b209-525bc6426f33", "uri": "../flows/a2b32f97-3fc7-4af2-b209-525bc6426f33.xml"}, "exchange direction": "OUTPUT", "other": {"anies": [{"name": "referenceToUnitGroupDataSet", "value": {"shortDescription": [{"value": "kg", "lang": "en"}], "type": "unit group data set", "refObjectId": "ad38d542-3fe9-439d-9b95-2f5f7752acaf", "uri": "../unitgroups/ad38d542-3fe9-439d-9b95-2f5f7752acaf.xml"}}, {"value": "0", "module": "A1-A3"}, {"value": "0", "module": "A4"}, {"value": "0", "module": "A5"}, {"value": "0", "module": "C1"}, {"value": "0", "module": "C2"}, {"value": "0", "module": "C3"}, {"value": "0", "module": "C4"}, {"value": "0", "module": "D"}]}, "resolvedFlowVersion": "38.00.000", "flowProperties": [], "typeOfFlow": "Other flow", "classification": {"classHierarchy": "Quantities / Environmental quantities / EPD EN 15804 / LCI indicators", "name": "GaBiCategories"}}, {"dataSetInternalID": 15, "referenceToFlowDataSet": {"shortDescription": [{"value": "Materials for recycling (MFR)", "lang": "en"}, {"value": "Stoffe zum Recycling (MFR)", "lang": "de"}], "type": "flow data set", "refObjectId": "d7fe48a5-4103-49c8-9aae-b0b5dfdbd6ae", "uri": "../flows/d7fe48a5-4103-49c8-9aae-b0b5dfdbd6ae.xml"}, "exchange direction": "OUTPUT", "other": {"anies": [{"name": "referenceToUnitGroupDataSet", "value": {"shortDescription": [{"value": "kg", "lang": "en"}], "type": "unit group data set", "refObjectId": "ad38d542-3fe9-439d-9b95-2f5f7752acaf", "uri": "../unitgroups/ad38d542-3fe9-439d-9b95-2f5f7752acaf.xml"}}, {"value": "0", "module": "A1-A3"}, {"value": "0", "module": "A4"}, {"value": "0", "module": "A5"}, {"value": "0", "module": "C1"}, {"value": "0", "module": "C2"}, {"value": "0", "module": "C3"}, {"value": "0", "module": "C4"}, {"value": "0", "module": "D"}]}, "resolvedFlowVersion": "38.00.000", "flowProperties": [], "typeOfFlow": "Other flow", "classification": {"classHierarchy": "Quantities / Environmental quantities / EPD EN 15804 / LCI indicators", "name": "GaBiCategories"}}, {"dataSetInternalID": 16, "referenceToFlowDataSet": {"shortDescription": [{"value": "Materials for energy recovery (MER)", "lang": "en"}, {"value": "Stoffe für die Energierückgewinnung (MER)", "lang": "de"}], "type": "flow data set", "refObjectId": "59a9181c-3aaf-46ee-8b13-2b3723b6e447", "uri": "../flows/59a9181c-3aaf-46ee-8b13-2b3723b6e447.xml"}, "exchange direction": "OUTPUT", "other": {"anies": [{"name": "referenceToUnitGroupDataSet", "value": {"shortDescription": [{"value": "kg", "lang": "en"}], "type": "unit group data set", "refObjectId": "ad38d542-3fe9-439d-9b95-2f5f7752acaf", "uri": "../unitgroups/ad38d542-3fe9-439d-9b95-2f5f7752acaf.xml"}}, {"value": "0", "module": "A1-A3"}, {"value": "0", "module": "A4"}, {"value": "57.336", "module": "A5"}, {"value": "0", "module": "C1"}, {"value": "0", "module": "C2"}, {"value": "0", "module": "C3"}, {"value": "594.861", "module": "C4"}, {"value": "0", "module": "D"}]}, "resolvedFlowVersion": "38.00.000", "flowProperties": [], "typeOfFlow": "Other flow", "classification": {"classHierarchy": "Quantities / Environmental quantities / EPD EN 15804 / LCI indicators", "name": "GaBiCategories"}}, {"dataSetInternalID": 17, "referenceToFlowDataSet": {"shortDescription": [{"value": "Exported electrical energy (EEE)", "lang": "en"}, {"value": "Exportierte elektrische Energie (EEE)", "lang": "de"}], "type": "flow data set", "refObjectId": "4da0c987-2b76-40d6-9e9e-82a017aaaf29", "uri": "../flows/4da0c987-2b76-40d6-9e9e-82a017aaaf29.xml"}, "exchange direction": "OUTPUT", "other": {"anies": [{"name": "referenceToUnitGroupDataSet", "value": {"shortDescription": [{"value": "MJ", "lang": "en"}], "type": "unit group data set", "refObjectId": "93a60a57-a3c8-11da-a746-0800200c9a66", "uri": "../unitgroups/93a60a57-a3c8-11da-a746-0800200c9a66.xml"}}, {"value": "0", "module": "A1-A3"}, {"value": "0", "module": "A4"}, {"value": "0", "module": "A5"}, {"value": "0", "module": "C1"}, {"value": "0", "module": "C2"}, {"value": "0", "module": "C3"}, {"value": "0", "module": "C4"}, {"value": "0", "module": "D"}]}, "resolvedFlowVersion": "38.00.000", "flowProperties": [], "typeOfFlow": "Other flow", "classification": {"classHierarchy": "Quantities / Environmental quantities / EPD EN 15804 / LCI indicators", "name": "GaBiCategories"}}, {"dataSetInternalID": 18, "referenceToFlowDataSet": {"shortDescription": [{"value": "Exported thermal energy (EET)", "lang": "en"}, {"value": "Exportierte thermische Energie (EET)", "lang": "de"}], "type": "flow data set", "refObjectId": "98daf38a-7a79-46d3-9a37-2b7bd0955810", "uri": "../flows/98daf38a-7a79-46d3-9a37-2b7bd0955810.xml"}, "exchange direction": "OUTPUT", "other": {"anies": [{"name": "referenceToUnitGroupDataSet", "value": {"shortDescription": [{"value": "MJ", "lang": "en"}], "type": "unit group data set", "refObjectId": "93a60a57-a3c8-11da-a746-0800200c9a66", "uri": "../unitgroups/93a60a57-a3c8-11da-a746-0800200c9a66.xml"}}, {"value": "0", "module": "A1-A3"}, {"value": "0", "module": "A4"}, {"value": "967.11642045564", "module": "A5"}, {"value": "0", "module": "C1"}, {"value": "0", "module": "C2"}, {"value": "0", "module": "C3"}, {"value": "8322.10539", "module": "C4"}, {"value": "0", "module": "D"}]}, "resolvedFlowVersion": "38.00.000", "flowProperties": [], "typeOfFlow": "Other flow", "classification": {"classHierarchy": "Quantities / Environmental quantities / EPD EN 15804 / LCI indicators", "name": "GaBiCategories"}}]}, "LCIAResults": {"LCIAResult": [{"referenceToLCIAMethodDataSet": {"shortDescription": [{"value": "Global Warming Potential total (GWP-total)", "lang": "en"}, {"value": "Globales Erwärmungspotenzial total (GWP-total)", "lang": "de"}], "type": "LCIA method data set", "refObjectId": "6a37f984-a4b3-458a-a20a-64418c145fa2", "uri": "../lciamethods/6a37f984-a4b3-458a-a20a-64418c145fa2.xml"}, "other": {"anies": [{"name": "referenceToUnitGroupDataSet", "value": {"shortDescription": [{"value": "kg CO_(2) eq", "lang": "en"}], "type": "unit group data set", "refObjectId": "1ebf3012-d0db-4de2-aefd-ef30cedb0be1", "uri": "../unitgroups/1ebf3012-d0db-4de2-aefd-ef30cedb0be1.xml"}}, {"value": "-781.120226567226", "module": "A1-A3"}, {"value": "26.7415318890957", "module": "A4"}, {"value": "93.7", "module": "A5"}, {"value": "0.0294604239481893", "module": "C1"}, {"value": "5.96289270569741", "module": "C2"}, {"value": "0", "module": "C3"}, {"value": "1040", "module": "C4"}, {"value": "-248.685749032336", "module": "D"}]}}, {"referenceToLCIAMethodDataSet": {"shortDescription": [{"value": "Global Warming Potential fossil fuels (GWP-fossil)", "lang": "en"}, {"value": "Globales Erwärmungspotenzial fossil (GWP-fossil)", "lang": "de"}], "type": "LCIA method data set", "refObjectId": "5f635281-343e-44fb-83df-1971b155e6b6", "uri": "../lciamethods/5f635281-343e-44fb-83df-1971b155e6b6.xml"}, "other": {"anies": [{"name": "referenceToUnitGroupDataSet", "value": {"shortDescription": [{"value": "kg CO_(2) eq", "lang": "en"}], "type": "unit group data set", "refObjectId": "1ebf3012-d0db-4de2-aefd-ef30cedb0be1", "uri": "../unitgroups/1ebf3012-d0db-4de2-aefd-ef30cedb0be1.xml"}}, {"value": "330.173658939049", "module": "A1-A3"}, {"value": "26.7047389078196", "module": "A4"}, {"value": "4.81657179883134", "module": "A5"}, {"value": "0.0284751145168615", "module": "C1"}, {"value": "5.95519561681463", "module": "C2"}, {"value": "0", "module": "C3"}, {"value": "6.46994774702051", "module": "C4"}, {"value": "-248.631806131107", "module": "D"}]}}, {"referenceToLCIAMethodDataSet": {"shortDescription": [{"value": "Global Warming Potential biogenic (GWP-biogenic)", "lang": "en"}, {"value": "Globales Erwärmungspotenzial biogen (GWP-biogenic)", "lang": "de"}], "type": "LCIA method data set", "refObjectId": "2356e1ab-0185-4db5-86e5-16de51c7485c", "uri": "../lciamethods/2356e1ab-0185-4db5-86e5-16de51c7485c.xml"}, "other": {"anies": [{"name": "referenceToUnitGroupDataSet", "value": {"shortDescription": [{"value": "kg CO_(2) eq", "lang": "en"}], "type": "unit group data set", "refObjectId": "1ebf3012-d0db-4de2-aefd-ef30cedb0be1", "uri": "../unitgroups/1ebf3012-d0db-4de2-aefd-ef30cedb0be1.xml"}}, {"value": "-1112.52344337036", "module": "A1-A3"}, {"value": "0.027190849547052", "module": "A4"}, {"value": "88.9", "module": "A5"}, {"value": "0.000918017303820079", "module": "C1"}, {"value": "0.00535838409654867", "module": "C2"}, {"value": "0", "module": "C3"}, {"value": "1030", "module": "C4"}, {"value": "-0.0461546258306625", "module": "D"}]}}, {"referenceToLCIAMethodDataSet": {"shortDescription": [{"value": "Global Warming Potential luluc (GWP-luluc)", "lang": "en"}, {"value": "Globales Erwärmungspotenzial luluc (GWP-luluc)", "lang": "de"}], "type": "LCIA method data set", "refObjectId": "4331bbdb-978a-490d-8707-eeb047f01a55", "uri": "../lciamethods/4331bbdb-978a-490d-8707-eeb047f01a55.xml"}, "other": {"anies": [{"name": "referenceToUnitGroupDataSet", "value": {"shortDescription": [{"value": "kg CO_(2) eq", "lang": "en"}], "type": "unit group data set", "refObjectId": "1ebf3012-d0db-4de2-aefd-ef30cedb0be1", "uri": "../unitgroups/1ebf3012-d0db-4de2-aefd-ef30cedb0be1.xml"}}, {"value": "1.2295423534437", "module": "A1-A3"}, {"value": "0.00960174992478384", "module": "A4"}, {"value": "0.00324165138386507", "module": "A5"}, {"value": "6.72891127207998E-05", "module": "C1"}, {"value": "0.00233860220697557", "module": "C2"}, {"value": "0", "module": "C3"}, {"value": "0.00218760719065082", "module": "C4"}, {"value": "-0.00778793917353552", "module": "D"}]}}, {"referenceToLCIAMethodDataSet": {"shortDescription": [{"value": "Depletion potential of the stratospheric ozone layer (ODP)", "lang": "en"}, {"value": "Abbau Potential der stratosphärischen Ozonschicht (ODP)", "lang": "de"}], "type": "LCIA method data set", "refObjectId": "b5c629d6-def3-11e6-bf01-fe55135034f3", "uri": "../lciamethods/b5c629d6-def3-11e6-bf01-fe55135034f3.xml"}, "other": {"anies": [{"name": "referenceToUnitGroupDataSet", "value": {"shortDescription": [{"value": "kg CFC11 eq", "lang": "en"}], "type": "unit group data set", "refObjectId": "d9e957c9-7309-4474-bf3a-7777df6c4e5b", "uri": "../unitgroups/d9e957c9-7309-4474-bf3a-7777df6c4e5b.xml"}}, {"value": "3.9352957750862E-05", "module": "A1-A3"}, {"value": "6.37780448026613E-06", "module": "A4"}, {"value": "4.06626569977194E-07", "module": "A5"}, {"value": "1.43545364604935E-09", "module": "C1"}, {"value": "1.3782562697987E-06", "module": "C2"}, {"value": "0", "module": "C3"}, {"value": "1.01230699329167E-06", "module": "C4"}, {"value": "-3.48566209119256E-05", "module": "D"}]}}, {"referenceToLCIAMethodDataSet": {"shortDescription": [{"value": "Acidification potential of land and water (AP)", "lang": "en"}, {"value": "Versauerungspotenzial von Boden und Wasser (AP)", "lang": "de"}], "type": "LCIA method data set", "refObjectId": "b5c611c6-def3-11e6-bf01-fe55135034f3", "uri": "../lciamethods/b5c611c6-def3-11e6-bf01-fe55135034f3.xml"}, "other": {"anies": [{"name": "referenceToUnitGroupDataSet", "value": {"shortDescription": [{"value": "mol H^(+) eq", "lang": "en"}], "type": "unit group data set", "refObjectId": "42e089ac-92bf-4bf2-8ca1-5fc40d18f2ed", "uri": "../unitgroups/42e089ac-92bf-4bf2-8ca1-5fc40d18f2ed.xml"}}, {"value": "1.81787300587928", "module": "A1-A3"}, {"value": "0.111440371194706", "module": "A4"}, {"value": "0.0352464737778308", "module": "A5"}, {"value": "0.000162017560436078", "module": "C1"}, {"value": "0.0241671822392883", "module": "C2"}, {"value": "0", "module": "C3"}, {"value": "0.192947374153375", "module": "C4"}, {"value": "-0.320495305774495", "module": "D"}]}}, {"referenceToLCIAMethodDataSet": {"shortDescription": [{"value": "Eutrophication potential aquatic freshwater (EP-freshwater)", "lang": "en"}, {"value": "Eutrophierungspotenzial Süßwasser (EP-freshwater)", "lang": "de"}], "type": "LCIA method data set", "refObjectId": "b53ec18f-7377-4ad3-86eb-cc3f4f276b2b", "uri": "../lciamethods/b53ec18f-7377-4ad3-86eb-cc3f4f276b2b.xml"}, "other": {"anies": [{"name": "referenceToUnitGroupDataSet", "value": {"shortDescription": [{"value": "kg P eq", "lang": "en"}], "type": "unit group data set", "refObjectId": "0429039d-a61d-4590-ba67-aa4a20a810a1", "uri": "../unitgroups/0429039d-a61d-4590-ba67-aa4a20a810a1.xml"}}, {"value": "0.0155064291339301", "module": "A1-A3"}, {"value": "0.000182607443579752", "module": "A4"}, {"value": "0.000185867938140315", "module": "A5"}, {"value": "3.04141474704143E-06", "module": "C1"}, {"value": "4.17505560314392E-05", "module": "C2"}, {"value": "0", "module": "C3"}, {"value": "0.000109762091079815", "module": "C4"}, {"value": "-0.00022733646269118", "module": "D"}]}}, {"referenceToLCIAMethodDataSet": {"shortDescription": [{"value": "Eutrophication potential aquatic marine (EP-marine)", "lang": "en"}, {"value": "Eutrophierungspotenzial Salzwasser (EP-marine)", "lang": "de"}], "type": "LCIA method data set", "refObjectId": "b5c619fa-def3-11e6-bf01-fe55135034f3", "uri": "../lciamethods/b5c619fa-def3-11e6-bf01-fe55135034f3.xml"}, "other": {"anies": [{"name": "referenceToUnitGroupDataSet", "value": {"shortDescription": [{"value": "kg N eq", "lang": "en"}], "type": "unit group data set", "refObjectId": "d05bb823-ecdf-4686-8c40-bf1d9257859f", "uri": "../unitgroups/d05bb823-ecdf-4686-8c40-bf1d9257859f.xml"}}, {"value": "0.279220907608811", "module": "A1-A3"}, {"value": "0.0336704227779295", "module": "A4"}, {"value": "0.0125507823459965", "module": "A5"}, {"value": "2.0664456825598E-05", "module": "C1"}, {"value": "0.00720617407092639", "module": "C2"}, {"value": "0", "module": "C3"}, {"value": "0.0932003903121769", "module": "C4"}, {"value": "-0.116327618464239", "module": "D"}]}}, {"referenceToLCIAMethodDataSet": {"shortDescription": [{"value": "Eutrophication potential terrestrial (EP-terrestrial)", "lang": "en"}, {"value": "Eutrophierungspotenzial Land (EP-terrestrial)", "lang": "de"}], "type": "LCIA method data set", "refObjectId": "b5c614d2-def3-11e6-bf01-fe55135034f3", "uri": "../lciamethods/b5c614d2-def3-11e6-bf01-fe55135034f3.xml"}, "other": {"anies": [{"name": "referenceToUnitGroupDataSet", "value": {"shortDescription": [{"value": "mol N eq", "lang": "en"}], "type": "unit group data set", "refObjectId": "71b4d617-0ec9-4d3f-b65e-e438940c2401", "uri": "../unitgroups/71b4d617-0ec9-4d3f-b65e-e438940c2401.xml"}}, {"value": "4.34069735604762", "module": "A1-A3"}, {"value": "0.371728912698735", "module": "A4"}, {"value": "0.133967466244172", "module": "A5"}, {"value": "0.000238149712116707", "module": "C1"}, {"value": "0.0795613944342524", "module": "C2"}, {"value": "0", "module": "C3"}, {"value": "1.0268001719667", "module": "C4"}, {"value": "-1.27537574189852", "module": "D"}]}}, {"referenceToLCIAMethodDataSet": {"shortDescription": [{"value": "Formation potential of tropospheric ozone photochemical oxidants (POCP)", "lang": "en"}, {"value": "Bildungspotential für troposphärisches Ozon (POCP)", "lang": "de"}], "type": "LCIA method data set", "refObjectId": "b5c610fe-def3-11e6-bf01-fe55135034f3", "uri": "../lciamethods/b5c610fe-def3-11e6-bf01-fe55135034f3.xml"}, "other": {"anies": [{"name": "referenceToUnitGroupDataSet", "value": {"shortDescription": [{"value": "kg NMVOC eq", "lang": "en"}], "type": "unit group data set", "refObjectId": "d27c25f8-fbc1-44c6-b47b-4adbae4199c6", "uri": "../unitgroups/d27c25f8-fbc1-44c6-b47b-4adbae4199c6.xml"}}, {"value": "1.40919956017177", "module": "A1-A3"}, {"value": "0.119624541548213", "module": "A4"}, {"value": "0.0420040797942961", "module": "A5"}, {"value": "6.54343888069451E-05", "module": "C1"}, {"value": "0.0243659191501349", "module": "C2"}, {"value": "0", "module": "C3"}, {"value": "0.272182869318493", "module": "C4"}, {"value": "-0.436536756742249", "module": "D"}]}}, {"referenceToLCIAMethodDataSet": {"shortDescription": [{"value": "Abiotic depletion potential for non fossil resources (ADPE)", "lang": "en"}, {"value": "Potenzial für den abiotischen Abbau nicht fossiler Ressourcen (ADPE)", "lang": "de"}], "type": "LCIA method data set", "refObjectId": "b2ad6494-c78d-11e6-9d9d-cec0c932ce01", "uri": "../lciamethods/b2ad6494-c78d-11e6-9d9d-cec0c932ce01.xml"}, "other": {"anies": [{"name": "referenceToUnitGroupDataSet", "value": {"shortDescription": [{"value": "kg Sb eq", "lang": "en"}], "type": "unit group data set", "refObjectId": "54ccd2d9-a32a-4fc2-923d-f2c8c93e89d4", "uri": "../unitgroups/54ccd2d9-a32a-4fc2-923d-f2c8c93e89d4.xml"}}, {"value": "0.00381587555031457", "module": "A1-A3"}, {"value": "6.12379637524087E-05", "module": "A4"}, {"value": "4.89861280910926E-05", "module": "A5"}, {"value": "2.6757704552618E-07", "module": "C1"}, {"value": "2.07092187056872E-05", "module": "C2"}, {"value": "0", "module": "C3"}, {"value": "2.32264336256061E-05", "module": "C4"}, {"value": "-0.000146945999752575", "module": "D"}]}}, {"referenceToLCIAMethodDataSet": {"shortDescription": [{"value": "Abiotic depletion potential for fossil resources (ADPF)", "lang": "en"}, {"value": "Potenzial für den abiotischen Abbau fossiler Brennstoffe (ADPF)", "lang": "de"}], "type": "LCIA method data set", "refObjectId": "b2ad6110-c78d-11e6-9d9d-cec0c932ce01", "uri": "../lciamethods/b2ad6110-c78d-11e6-9d9d-cec0c932ce01.xml"}, "other": {"anies": [{"name": "referenceToUnitGroupDataSet", "value": {"shortDescription": [{"value": "MJ", "lang": "en"}], "type": "unit group data set", "refObjectId": "93a60a57-a3c8-11da-a746-0800200c9a66", "uri": "../unitgroups/93a60a57-a3c8-11da-a746-0800200c9a66.xml"}}, {"value": "5589.71763954847", "module": "A1-A3"}, {"value": "416.256775892601", "module": "A4"}, {"value": "53.8929070786381", "module": "A5"}, {"value": "0.60672603848248", "module": "C1"}, {"value": "90.0427181710172", "module": "C2"}, {"value": "0", "module": "C3"}, {"value": "83.2166789862594", "module": "C4"}, {"value": "-3476.26673208641", "module": "D"}]}}, {"referenceToLCIAMethodDataSet": {"shortDescription": [{"value": "Water use (WDP)", "lang": "en"}, {"value": "Wassernutzung (WDP)", "lang": "de"}], "type": "LCIA method data set", "refObjectId": "b2ad66ce-c78d-11e6-9d9d-cec0c932ce01", "uri": "../lciamethods/b2ad66ce-c78d-11e6-9d9d-cec0c932ce01.xml"}, "other": {"anies": [{"name": "referenceToUnitGroupDataSet", "value": {"shortDescription": [{"value": "m^(3) world eq deprived", "lang": "en"}], "type": "unit group data set", "refObjectId": "6ae2df01-888e-46c8-b17d-49fa3869b476", "uri": "../unitgroups/6ae2df01-888e-46c8-b17d-49fa3869b476.xml"}}, {"value": "429.062739848131", "module": "A1-A3"}, {"value": "1.43215536946329", "module": "A4"}, {"value": "1.06302786038123", "module": "A5"}, {"value": "0.00708982951742961", "module": "C1"}, {"value": "0.269641602529168", "module": "C2"}, {"value": "0", "module": "C3"}, {"value": "1.86380242894479", "module": "C4"}, {"value": "-1.42050350680927", "module": "D"}]}}, {"referenceToLCIAMethodDataSet": {"shortDescription": [{"value": "Incidence of disease due to PM emissions (PM)", "lang": "en"}, {"value": "Auftreten von Krankheiten aufgrund von Feinstaubemissionen (PM)", "lang": "de"}], "type": "LCIA method data set", "refObjectId": "b5c602c6-def3-11e6-bf01-fe55135034f3", "uri": "../lciamethods/b5c602c6-def3-11e6-bf01-fe55135034f3.xml"}, "other": {"anies": [{"name": "referenceToUnitGroupDataSet", "value": {"shortDescription": [{"value": "Disease incidence", "lang": "en"}], "type": "unit group data set", "refObjectId": "3883559b-648f-4afc-8ba2-0bd24f3affa3", "uri": "../unitgroups/3883559b-648f-4afc-8ba2-0bd24f3affa3.xml"}}, {"value": "6.81709842370693E-05", "module": "A1-A3"}, {"value": "3.1358135154203E-06", "module": "A4"}, {"value": "4.9615146601772E-07", "module": "A5"}, {"value": "4.47952970365297E-10", "module": "C1"}, {"value": "5.12464884773823E-07", "module": "C2"}, {"value": "0", "module": "C3"}, {"value": "1.67742456311346E-06", "module": "C4"}, {"value": "-9.9652547711952E-07", "module": "D"}]}}, {"referenceToLCIAMethodDataSet": {"shortDescription": [{"value": "Human exposure efficiency relative to U235 (IR)", "lang": "en"}, {"value": "Wirkung durch Exposition des Menschen mit U235 (IR)", "lang": "de"}], "type": "LCIA method data set", "refObjectId": "b5c632be-def3-11e6-bf01-fe55135034f3", "uri": "../lciamethods/b5c632be-def3-11e6-bf01-fe55135034f3.xml"}, "other": {"anies": [{"name": "referenceToUnitGroupDataSet", "value": {"shortDescription": [{"value": "kBq U235 eq", "lang": "en"}], "type": "unit group data set", "refObjectId": "456b05bf-1415-44a9-9993-02452f554c09", "uri": "../unitgroups/456b05bf-1415-44a9-9993-02452f554c09.xml"}}, {"value": "7.63104250815503", "module": "A1-A3"}, {"value": "1.80521000287331", "module": "A4"}, {"value": "0.144151985687689", "module": "A5"}, {"value": "0.00545236660904475", "module": "C1"}, {"value": "0.390922675937457", "module": "C2"}, {"value": "0", "module": "C3"}, {"value": "0.242625951997314", "module": "C4"}, {"value": "-0.326315376273068", "module": "D"}]}}, {"referenceToLCIAMethodDataSet": {"shortDescription": [{"value": "Comparative toxic unit for ecosystems (ETP-fw)", "lang": "en"}, {"value": "Toxizitätsvergleichseinheit für Ökosysteme (ETP-fw)", "lang": "de"}], "type": "LCIA method data set", "refObjectId": "ee1082d1-b0f7-43ca-a1f0-21e2a4a74511", "uri": "../lciamethods/ee1082d1-b0f7-43ca-a1f0-21e2a4a74511.xml"}, "other": {"anies": [{"name": "referenceToUnitGroupDataSet", "value": {"shortDescription": [{"value": "CTUe", "lang": "en"}], "type": "unit group data set", "refObjectId": "aa959ded-f1eb-4efb-9c5c-2d60be36b3e6", "uri": "../unitgroups/aa959ded-f1eb-4efb-9c5c-2d60be36b3e6.xml"}}, {"value": "7115.16214623181", "module": "A1-A3"}, {"value": "325.152027322437", "module": "A4"}, {"value": "134.154929563778", "module": "A5"}, {"value": "0.383806196754041", "module": "C1"}, {"value": "70.2748840877183", "module": "C2"}, {"value": "0", "module": "C3"}, {"value": "149.232623275137", "module": "C4"}, {"value": "-279.764800862409", "module": "D"}]}}, {"referenceToLCIAMethodDataSet": {"shortDescription": [{"value": "Comparative toxic unit for humans (carcinogenic) (HTP-c)", "lang": "en"}, {"value": "Toxizitätsvergleichseinheit für Menschen (krebserregend) (HTP-c)", "lang": "de"}], "type": "LCIA method data set", "refObjectId": "2299222a-bbd8-474f-9d4f-4dd1f18aea7c", "uri": "../lciamethods/2299222a-bbd8-474f-9d4f-4dd1f18aea7c.xml"}, "other": {"anies": [{"name": "referenceToUnitGroupDataSet", "value": {"shortDescription": [{"value": "CTUh", "lang": "en"}], "type": "unit group data set", "refObjectId": "d4c9523e-2d7e-49fd-8469-998f547d3a70", "uri": "../unitgroups/d4c9523e-2d7e-49fd-8469-998f547d3a70.xml"}}, {"value": "5.2689924267115E-07", "module": "A1-A3"}, {"value": "8.99426325624105E-09", "module": "A4"}, {"value": "4.39985054862187E-08", "module": "A5"}, {"value": "1.18132223016896E-11", "module": "C1"}, {"value": "2.27591258647363E-09", "module": "C2"}, {"value": "0", "module": "C3"}, {"value": "1.77567180677089E-07", "module": "C4"}, {"value": "-1.49571570302344E-08", "module": "D"}]}}, {"referenceToLCIAMethodDataSet": {"shortDescription": [{"value": "Comparative toxic unit for humans (noncarcinogenic) (HTP-nc)", "lang": "en"}, {"value": "Toxizitätsvergleichseinheit für Menschen (nicht krebserregend) (HTP-nc)", "lang": "de"}], "type": "LCIA method data set", "refObjectId": "3af763a5-b7a1-48c9-9cee-1f223481fcef", "uri": "../lciamethods/3af763a5-b7a1-48c9-9cee-1f223481fcef.xml"}, "other": {"anies": [{"name": "referenceToUnitGroupDataSet", "value": {"shortDescription": [{"value": "CTUh", "lang": "en"}], "type": "unit group data set", "refObjectId": "d4c9523e-2d7e-49fd-8469-998f547d3a70", "uri": "../unitgroups/d4c9523e-2d7e-49fd-8469-998f547d3a70.xml"}}, {"value": "7.65445428718617E-06", "module": "A1-A3"}, {"value": "3.55819660291765E-07", "module": "A4"}, {"value": "1.75622307304943E-07", "module": "A5"}, {"value": "3.76887449313472E-10", "module": "C1"}, {"value": "7.36847315648072E-08", "module": "C2"}, {"value": "0", "module": "C3"}, {"value": "5.4105532324487E-07", "module": "C4"}, {"value": "-7.84746182645755E-07", "module": "D"}]}}, {"referenceToLCIAMethodDataSet": {"shortDescription": [{"value": "Soil quality index (SQP)", "lang": "en"}, {"value": "Bodenqualitätsindex (SQP)", "lang": "de"}], "type": "LCIA method data set", "refObjectId": "b2ad6890-c78d-11e6-9d9d-cec0c932ce01", "uri": "../lciamethods/b2ad6890-c78d-11e6-9d9d-cec0c932ce01.xml"}, "other": {"anies": [{"name": "referenceToUnitGroupDataSet", "value": {"shortDescription": [{"value": "SQP", "lang": "en"}], "type": "unit group data set", "refObjectId": "f130951c-e67f-4f7f-8dd4-665de3974e18", "uri": "../unitgroups/f130951c-e67f-4f7f-8dd4-665de3974e18.xml"}}, {"value": "33550.9314145584", "module": "A1-A3"}, {"value": "476.272641676055", "module": "A4"}, {"value": "28.8676398829423", "module": "A5"}, {"value": "0.109609873633754", "module": "C1"}, {"value": "61.8636962051859", "module": "C2"}, {"value": "0", "module": "C3"}, {"value": "87.9353902659942", "module": "C4"}, {"value": "-68.0001121646186", "module": "D"}]}}]}, "otherAttributes": {"{http://www.indata.network/EPD/2019}epd-version": "1.2"}, "version": "1.1", "locations": "../ILCDLocations.xml"}