{"processInformation": {"dataSetInformation": {"UUID": "de2e3dc4-8687-4bf9-9cd1-c7ed51bfe3a2", "name": {"baseName": [{"value": "Products based on polyurethane or silane-modified polymer, group 2", "lang": "en"}, {"value": "Produkte auf Basis Polyurethan oder silanmodifiziertem Polymer, Gruppe 2", "lang": "de"}], "functionalUnitFlowProperties": [{"lang": "en"}]}, "classificationInformation": {"classification": [{"class": [{"value": "Beschichtungen", "level": 0, "classId": "5"}, {"value": "Reaktionsharze", "level": 1, "classId": "5.8"}, {"value": "Reaktionsharze auf PU-Basis", "level": 2, "classId": "5.8.02"}], "name": "OEKOBAU.DAT"}, {"class": [{"value": "02 Building products", "level": 0}, {"value": "Construction adhesives and coatings", "level": 1}, {"value": "Reaction resin products", "level": 2}], "name": "IBUCategories"}]}, "generalComment": [{"value": "This EPD comprises reactive products based on polyurethane (PU) or silane-modified polymer (SMP) with a volatile organic compound (VOC) content ≤1 % (VOC definition according to Decopaint Directive) and a castor oil/-derivatives content ≤10 %. The one- or two-component reactive PU products are manufactured using polyols and isocyanates. Reactive products based on SMP polymers are usually manufactured as a one-component system from polyols and alkoxysilane in a preliminary stage. The aqueous systems consist of (a) dispersion and are crosslinked by a dispersible isocyanate. The products fulfil manifold, often specific, functions in the construction, furnishing and repair of buildings. The product displaying the highest environmental impacts was used as a representative product for calculating the Life Cycle Assessment results (worst-case approach).", "lang": "en"}]}, "quantitativeReference": {"referenceToReferenceFlow": [0]}, "time": {"referenceYear": 2022, "dataSetValidUntil": 2027, "other": {"anies": [{"name": "publicationDateOfEPD", "value": 1654041600000}]}}, "geography": {"locationOfOperationSupplyOrProduction": {"location": "RER"}}, "technology": {"technologyDescriptionAndIncludedProcesses": [{"value": "This EPD comprises reactive products based on polyurethane (PU) or silane-modified polymer (SMP) with a volatile organic copound (VOC) content ≤1 % (VOC definition according to Decopaint Directive) and a castor oil/-derivatives content ≤ 10%. The one- or two-component reactive PU products are manufactured using polyols and isocyanates. Reactive products based on SMP polymers are usually manufactured as a one-component system from polyols and alkoxysilane in a preliminary stage. The aqueous systems consist of (a) dispersion and are crosslinked by a dispersible isocyanate. The products fulfil manifold, often specific, functions in the construction, furnishing and repair of buildings. According to the Model EPD system (IBU) and the guideline and the substance list (available for members of the trade associations FEICA, EFCC, IVK and DBC), the environmental impacts of the substances are condensed to a single score; the single score of a formulation is calculated based on the single score of the substances. The products are grouped according to their single score (group 1 to 6), the formulation displaying the highest environmental impacts was used as a representative product for calculating the Life Cycle Assessment results (worst-case approach). \nTechnical data: \nThe density of the products is between 0,85 and 1,8 g/cm³, other relevant technical data can be found in the manufacturer’s technical documentation.\n\nModule 1: Reactive products as adhesive for parquet and floor coverings\n\nThe minimum requirements of EN ISO 17178 and EN ISO 22636 must be maintained.\n\n\nModule 2: Reactive products for protecting and repairing concrete structures \n\n2.1 The requirements on essential characteristics for all intended uses in accordance with EN 1504-2, Tables 1 and 5 must be maintained. These are:\n\n- Permeability to CO2 (EN 1062-6) \n\n- Water vapour permeability (EN ISO 7783-1/-2) \n\n- Capillary absorption and permeability to water (EN 1062-3) \n\n- Adhesive strength by pull-off test (EN 1542) \n\n2.2 Essential characteristics for all intended uses in accordance with EN 1504-4, Tables 3.1 and 3.2 (manufacturer's declaration of performance) \n\n2.3 Requirements on essential characteristics for all intended uses in accordance with EN 1504-5, Table 3: \n\n- Injectability (EN 1771) \n\n- Viscosity (EN ISO 3219) \n\nFurther essential characteristics in accordance with the manufacturer's technical documentation / declaration of performance\n\n\nModule 3:  Liquid-applied roof waterproofing kits \n\nThe minimum requirements of EAD 030350-00-0402 Liquid-applied roof waterproofing kits must be maintained. The essential characteristics are to be specified in accordance with the European Technical Assessment (ETA, specification no.).\n\n\nModule 4: Reactive products for liquid-applied bridge deck waterproofing kits \n\nThe minimum requirements of ETAG 033 Liquid-applied bridge deck waterproofing kits must be maintained. The essential characteristics are to be specified in accordance with the European Technical Assessment (ETA, specification no.).\n\n\nModule 5: Screed material, floor screeds and decorative floors \n\nThe requirements on essential characteristics according to EN 13813 'Screed material and floor screeds – Screed materials – Properties and requirements'/ must be maintained. For synthetic resin screeds, these are: \n\n- Bond strength (EN 13892-8) \n\n- Reaction to fire (EN 13501-1) \n\nFurther essential characteristics in accordance with the manufacturer's technical documentation/declaration of performance\n\n\nModule 6: Reactive products as an adhesive for tiles \n\nThe requirements on essential characteristics according to EN12004, must be maintained. These are:\n\n-Tensile adhesion strength after dry storage (EN 12004-2)\n\n-Tensile adhesion strength after water immersion (EN 12004-2)\n\n-Tensile adhesion strength after heat ageing (EN 12004-2)\n\n-Tensile adhesion strength after freeze/thaw cycles (EN 12004-2)\n\n-Open time: Tensile strength (EN 12004-2)\n\nFurther essential characteristics in accordance with the manufacturer's technical documentation \n\n\nModule 7: Adhesives and sealants \n\nPerformance characteristics in accordance with the manufacturer's technical documentation/declaration of performance  \n\n\nModule 8: Reactive products for watertight covering kits \n\nThe minimum requirements of EAD 030352-00-0503 Liquid applied watertight covering kits for wet room floors and/or walls must be maintained. The essential characteristics are to be specified in accordance with the European Technical Assessment (ETA, specification no.).\n\n\nModule 9: Reactive products for liquid-applied waterproofings\n\nThe minimum requirements of the test principles regarding the issuing of general building authority test certificates for liquid-applied products for waterproofing of buildings (PG-FLK) must be maintained. The characteristics for the proof of usability are to be specified in accordance with the test principles for granting general building authority test certificates for liquid applied polymer products for waterproofing buildings \n\n\nModule 10: Reactive products for waterproofing and/or for pre-treating mineral substrates \nDeclared unit: \nThis EPD refers to the declared unit of 1 kg of product based on polyurethane or silane-modified polymer, group 2; applied into the building with a density of 0.85 - 1.8 g/cm³ in accordance with the IBU PCR part B for reaction resin products.  \n\nThe results of the Life Cycle Assessment provided in this declaration have been selected from the product with the highest environmental impact (worst-case scenario).  \n\nDepending on the application, a corresponding conversion factor such as the density to convert volumetric use to mass must be taken into consideration. \n\n\nThe Declaration type is according to EN 15804: Cradle to gate with options, modules C1–C3, and module D (A1–A3, C, D) and additional modules.", "lang": "en"}, {"value": "Diese EPD umfasst reaktive Produkte auf Basis von Polyurethan (PU) oder silanmodifiziertem Polymer (SMP) mit einem Gehalt an flüchtigen organischen Verbindungen (VOC) ≤1 % (VOC-Definition gemäß Decopaint-Richtlinie) und einem Gehalt an Rizinusöl/-derivaten ≤ 10%. Die ein- oder zweikomponentigen reaktiven PU-Produkte werden unter Verwendung von Polyolen und Isocyanaten hergestellt. Reaktive Produkte auf Basis von SMP-Polymeren werden in der Regel als Einkomponentensystem aus Polyolen und Alkoxysilan in einer Vorstufe hergestellt. Die wässrigen Systeme bestehen aus (einer) Dispersion und werden durch ein dispergierbares Isocyanat vernetzt. Die Produkte erfüllen vielfältige, oft spezifische Funktionen beim Bau, der Einrichtung und der Instandsetzung von Gebäuden.\nNach dem Modell-EPD-System (IBU) und dem Leitfaden und der Stoffliste (erhältlich für Mitglieder der Fachverbände FEICA, EFCC, IVK und DBC) werden die Umweltauswirkungen der Stoffe zu einem Single Score verdichtet; der Single Score einer Formulierung wird auf der Basis des Single Scores der Stoffe berechnet. Die Produkte werden entsprechend ihrer Einzelpunktzahl in Gruppen eingeteilt (Gruppe 1 bis 6), wobei die Formulierung mit den höchsten Umweltauswirkungen als repräsentatives Produkt für die Berechnung der Ökobilanzergebnisse verwendet wurde (Worst-Case-Ansatz). \n", "lang": "de"}], "technologicalApplicability": [{"value": "Products based on polyurethane or silane-modified polymer, group 2, are used for the following applications:  \n\n Module 1: Adhesives for parquet and floor coverings\n Parquet adhesives in accordance with EN ISO 17178 for wooden and parquet floors and flooring adhesives in accordance with EN ISO 22636 for floor coverings \n\n Module 2: Reactive products for protecting and repairing concrete structures\n Products for increasing the durability of concrete and reinforced concrete structures as well as for new concrete and for maintenance and repair work (requirements 2.1), products for structural bonding of strengthening materials to an existing concrete structure (requirements 2.2) and products for concrete injection for filling cracks, voids and interstices in concrete (requirements 2.3) \n\n Module 3: Liquid-applied roof waterproofing kits\n Reactive products for waterproofing roof constructions which are applied on site \n\n Module 4: Reactive products for liquid-applied bridge deck waterproofing kits\n Products for liquid-applied waterproofing for use on concrete bridge decks \n\n Module 5: Screed material, floor screeds and decorative floors\n Products for screed/synthetic resin screed for use in floor constructions \n\n Module 6: Reactive products as an adhesive for tiles\n Tile adhesives for internal and external tile installations on walls, floors and ceilings \n\n Module 7: Adhesives and sealants\n Reactive products for use as:\n · Structural and repair adhesives\n · Surface and joint sealants\n Applications in accordance with the manufacturer's technical documentation/declaration of performance \n\n Module 8: Reactive products for watertight covering kits\n Products for waterproofing floors and/or walls in wet rooms inside buildings \n\n Module 9: Reactive products for liquid-applied waterproofing \n Liquid applied products for waterproofing of buildings \n\n Module 10: Reactive products for waterproofing and/or for pre-treating mineral substrates\n Applications in accordance with the manufacturer's technical documentation \n\n\nModule 11: Liquid-applied waterproofing membranes for use beneath ceramic tiling \n\n\nModule 12: One-component foam (OCF) \n\nOne component foam in a can is a one-component, \n\nself-expanding, ready to use polyurethane foam used \n\nfor various construction applications. It consists of a \n\nlow viscous semi-fluid in a can that leaves the can as a \n\nfroth and immediately forms a polyurethane foam. \n\n12.1 Window & External Door Sealing & Insulation: \n\nInstalling mechanically fixed external windows and \n\ndoors with an OCF, as part of a system including \n\nsealants and tapes \n\n12.2 Door Installation & Fixation: \n\nFixing interior doors with an OCF \n\n12.3 General Gap Filling: \n\nFilling of regularly and irregularly shaped spaces between at least two surfaces made of typical building materials with a one-component foam (OCF)\n\nModule 13: Sealants for glazing \n\nTwo-component reactive sealants are to be used as the second barrier of the structural hermetic seal in insulating glass units.\n\n\nModule 14: Bonded glazing sealants\n\n\nOne- and two-component reactive sealants are used for the bonding of insulating glass units in the window frame.", "lang": "en"}, {"value": "Produkte auf der Basis von Polyurethan oder silanmodifiziertem Polymer der Gruppe 2 werden für die folgenden Anwendungen eingesetzt: \n\n\nModul 1: Klebstoffe für Parkett und Bodenbeläge\nParkettklebstoffe nach EN ISO 17178 für Holz- und Parkettböden und Bodenbelagsklebstoffe nach EN ISO 22636 für Bodenbeläge\n\n\nModul 2: Reaktive Produkte für den Schutz und die Instandsetzung von Betonbauwerken\nProdukte zur Erhöhung der Dauerhaftigkeit von Beton- und Stahlbetonbauwerken sowie für neuen Beton und für Instandhaltungs- und Instandsetzungsarbeiten (Anforderungen 2.1), Produkte zum strukturellen Verbinden von Verstärkungsmaterialien mit einem bestehenden Betonbauwerk (Anforderungen 2.2) und Produkte zur Betoninjektion zum Füllen von Rissen, Hohlräumen und Zwischenräumen im Beton (Anforderungen 2.3)\n\n\nModul 3: Bausätze für flüssig aufzubringende Dachabdichtungen\nReaktive Produkte für die Abdichtung von Dachkonstruktionen, die vor Ort aufgebracht werden\n\n\nModul 4: Reaktive Produkte für flüssig aufzubringende Abdichtungen von Brückenfahrbahnen\nProdukte für flüssig aufzubringende Abdichtungen zur Verwendung auf Betonbrückenbelägen\n\n\nModul 5: Estrichmaterial, Estriche und dekorative Böden\nProdukte für Estrich/Kunstharzestrich zur Verwendung in Fußbodenkonstruktionen\n\n \nModul 6: Reaktive Produkte als Klebstoff für Fliesen\nFliesenkleber für die Innen- und Außenverlegung von Fliesen an Wänden, Böden und Decken\n\n \nModul 7: Klebstoffe und Dichtstoffe\nReaktive Produkte zur Verwendung als:\n- Konstruktions- und Reparaturklebstoffe\n- Flächen- und Fugendichtstoffe\nAnwendungen in Übereinstimmung mit der technischen Dokumentation/Leistungserklärung des Herstellers\n\n \nModul 8: Reaktive Produkte für wasserundurchlässige Abdeckungssätze\nProdukte für die Abdichtung von Böden und/oder Wänden in Feuchträumen innerhalb von Gebäuden\n\n \nModul 9: Reaktive Produkte für flüssig aufzubringende Abdichtungen\nFlüssig aufzubringende Produkte für die Abdichtung von Gebäuden\n\n\nModul 10: Reaktive Produkte für Abdichtungen und/oder zur Vorbehandlung von mineralischen Untergründen\nAnwendungen gemäß den technischen Unterlagen des Herstellers\n\n \n\nModul 11: Flüssig aufzubringende Abdichtungsbahnen für die Verwendung unter keramischen Fliesen und Platten\n\n \n\nModul 12: Einkomponentiger Schaum (OCF)\n\nEinkomponentenschaum in der Dose ist ein einkomponentiger,\n\nselbstexpandierender, gebrauchsfertiger Polyurethanschaum, der\n\nfür verschiedene Bauanwendungen. Er besteht aus einer\n\nniedrigviskosen Halbflüssigkeit in einer Dose, die die Dose als\n\nSchaum verlässt und sofort einen Polyurethanschaum bildet.\n\n12.1 Abdichtung und Isolierung von Fenstern und Außentüren:\n\nDer Einbau von mechanisch befestigten Außenfenstern und\n\nTüren mit einem OCF, als Teil eines Systems mit\n\nDichtstoffe und Bänder\n\n12.2 Einbau und Befestigung von Türen:\n\nBefestigung von Innentüren mit einer OCF\n\n12.3 Allgemeines Ausfüllen von Lücken:\n\nAusfüllen von regelmäßig und unregelmäßig geformten Zwischenräumen zwischen mindestens zwei Oberflächen aus typischen Baumaterialien mit einem Einkomponentenschaum (OCF)\n\n\n\nModul 13: Dichtstoffe für Verglasungen \n\nZweikomponenten-Reaktivdichtstoffe sind als zweite Barriere der strukturellen hermetischen Abdichtung in Isolierglaseinheiten zu verwenden.\n\n \n\nModul 14: Verglasungsdichtstoffe im Verbund\n\nEin- und Zweikomponenten-Reaktivdichtstoffe werden für die Verklebung von Isolierglaseinheiten im Fensterrahmen verwendet.", "lang": "de"}]}}, "modellingAndValidation": {"LCIMethodAndAllocation": {"typeOfDataSet": "EPD", "referenceToLCAMethodDetails": [{"shortDescription": [{"value": "Reaction resin products.pdf", "lang": "en"}], "type": "source data set", "refObjectId": "cf137026-621f-474e-9ae8-a42b6ffbe6ae"}], "other": {"anies": [{"name": "subType", "value": "template dataset"}]}}, "dataSourcesTreatmentAndRepresentativeness": {"referenceToDataSource": [{"shortDescription": [{"value": "GaBi Database (all versions)", "lang": "en"}], "type": "source data set", "refObjectId": "28d74cc0-db8b-4d7e-bc44-5f6d56ce0c4a"}, {"shortDescription": [{"value": "GaBi database SP40 2020", "lang": "en"}], "type": "source data set", "refObjectId": "0115289e-52f0-4920-bc7e-57b1c96aec8d"}], "useAdviceForDataSet": [{"value": "Scope: \nThis verified EPD entitles the holder to bear the symbol of the Institut Bauen und Umwelt e.V. It exclusively applies for products produced in Europe and for a period of five years from the date of issue. This EPD may be used by members of DBC, EFCC, FEICA and IVK and their members provided it has been proven that the respective product can be represented by this EPD. For this purpose a guideline is available at the secretariats of the four associations. The members of the associations are listed on the respective websites. \nSystem boundary: \nModules A1, A2 and A3 are taken into consideration in the LCA: \n\n-  A1 Production of preliminary products \n\n-  A2 Transport to the plant \n\n-  A3 Production incl. provision of energy, production of packaging as well as auxiliaries and consumables and waste treatment \n\n- A4 Transport to site \n\n- A5 Installation, product applied into the building during A5 phase operations and packaging disposal. This stage considers VOC emissions during the installation phase. The declared product does not contain substances in the formulation that directly emit (as) VOC, but VOCs are generated by a chemical reaction that are occurring during this phase. The end of life for the packaging material considered is described below: \n\n   -Incineration, for materials like plastic and wood. \n\n   -Landfill, for inert material like metals (where used). \n\n-C1-C2-C3-D \n\nThe building deconstruction (demolition process) takes place in the C1 module which considers energy production and consumption in terms of diesel and all the emissions connected with the fuel-burning process to run the machines. After the demolition, the product is transported to the end-of-life processing (C2 module) where all the impacts related to the transport processes are considered. For precautionary principle and as a worst-case scenario, thermal treatment  is the only end-of-life scenario considered. This is modelled by the incineration process (module C3) where the product ends its life cycle. Module D accounts for potential benefits that are beyond the defined system boundaries. Credits are generated during the incineration of wastes and related electricity produced that are occurring in the A5 module.", "lang": "en"}], "other": {"anies": [{"name": "referenceToOriginalEPD", "value": {"shortDescription": {"value": "Products based on polyurethane or silane-modified polymer, group 2.pdf", "defaultValue": "Products based on polyurethane or silane-modified polymer, group 2.pdf", "lstrings": [{"lang": "en", "value": "Products based on polyurethane or silane-modified polymer, group 2.pdf"}]}, "type": "source data set", "uuid": {"uuid": "7f3691d6-eed1-4a1c-9242-29055f128a17"}, "refObjectId": "7f3691d6-eed1-4a1c-9242-29055f128a17", "resourceURLs": ["https://oekobaudat.de/OEKOBAU.DAT/resource/sources/7f3691d6-eed1-4a1c-9242-29055f128a17/Products_based_on_polyurethane_or_silane-modified_polymer_group_2_15755.pdf?version=00.01.000"]}}]}}, "validation": {"review": [{"referenceToNameOfReviewerAndInstitution": [{"shortDescription": [{"value": "Institut Bauen und Umwelt e. V.", "lang": "en"}], "type": "contact data set", "refObjectId": "d111dbec-b024-4be5-86c5-752d6eb2cf95", "uri": "../contacts/d111dbec-b024-4be5-86c5-752d6eb2cf95.xml"}], "type": "Accredited third party review"}]}, "complianceDeclarations": {"compliance": [{"referenceToComplianceSystem": {"shortDescription": [{"value": "DIN EN 15804+A2", "lang": "en"}], "type": "source data set", "refObjectId": "c0016b33-8cf7-415c-ac6e-deba0d21440d", "uri": "../sources/c0016b33-8cf7-415c-ac6e-deba0d21440d.xml"}}, {"referenceToComplianceSystem": {"shortDescription": [{"value": "ISO 14025", "lang": "en"}], "type": "source data set", "refObjectId": "4f2eb655-6e44-4874-a95a-e28f5442cd4d", "uri": "../sources/4f2eb655-6e44-4874-a95a-e28f5442cd4d.xml"}}]}}, "administrativeInformation": {"commissionerAndGoal": {"referenceToCommissioner": [{"shortDescription": [{"value": "FEICA - Association of the European Adhesive and Sealant Industry", "lang": "en"}], "type": "contact data set", "refObjectId": "5fbf3785-e902-4624-8cdd-f257e972f20f", "uri": "../contacts/5fbf3785-e902-4624-8cdd-f257e972f20f.xml"}]}, "dataGenerator": {"referenceToPersonOrEntityGeneratingTheDataSet": [{"shortDescription": [{"value": "Sphera Solutions GmbH", "lang": "en"}], "type": "contact data set", "refObjectId": "623edf96-39d1-4e6f-9892-674c7228546b", "uri": "../contacts/623edf96-39d1-4e6f-9892-674c7228546b.xml"}]}, "dataEntryBy": {"timeStamp": 1654079352359, "referenceToDataSetFormat": [{"shortDescription": [{"value": "ILCD Format", "lang": "en"}], "type": "source data set", "refObjectId": "a97a0155-0234-4b87-b4ce-a45da52f2a40", "uri": "../sources/a97a0155-0234-4b87-b4ce-a45da52f2a40.xml"}, {"shortDescription": [{"value": "EPD-Datenformaterweiterungen v1.2", "lang": "de"}, {"value": "EPD Data Format Extensions v1.2", "lang": "en"}], "type": "source data set", "refObjectId": "a29449fd-aa2f-4de8-b5d7-4b06b43c6fde", "uri": "../sources/a29449fd-aa2f-4de8-b5d7-4b06b43c6fde.xml"}]}, "publicationAndOwnership": {"dataSetVersion": "00.02.000", "referenceToPrecedingDataSetVersion": [{"shortDescription": [{"value": "Reactive resins based on polyurethane or silane-modified polymer, unfilled/solvent-free, polyol-free ", "lang": "en"}], "type": "process data set", "refObjectId": "e830755d-e039-45a6-92b7-2cdbf7a71b90", "uri": "../processes/e830755d-e039-45a6-92b7-2cdbf7a71b90.xml"}], "referenceToRegistrationAuthority": {"shortDescription": [{"value": "Institut Bauen und Umwelt e. V.", "lang": "en"}], "type": "contact data set", "refObjectId": "d111dbec-b024-4be5-86c5-752d6eb2cf95", "uri": "../contacts/d111dbec-b024-4be5-86c5-752d6eb2cf95.xml"}, "registrationNumber": "EPD-FEI-20220106-IBG1-EN", "referenceToOwnershipOfDataSet": {"shortDescription": [{"value": "FEICA - Association of the European Adhesive and Sealant Industry", "lang": "en"}], "type": "contact data set", "refObjectId": "5fbf3785-e902-4624-8cdd-f257e972f20f", "uri": "../contacts/5fbf3785-e902-4624-8cdd-f257e972f20f.xml"}, "copyright": true, "licenseType": "Free of charge for all users and uses", "accessRestrictions": [{"value": "None", "lang": "en"}], "other": {"anies": [{"name": "referenceToPublisher", "value": {"shortDescription": [{"value": "Institut Bauen und Umwelt e. V.", "lang": "en"}], "type": "contact data set", "refObjectId": "d111dbec-b024-4be5-86c5-752d6eb2cf95", "uri": "../contacts/d111dbec-b024-4be5-86c5-752d6eb2cf95.xml"}}]}}}, "exchanges": {"exchange": [{"dataSetInternalID": 0, "referenceToFlowDataSet": {"shortDescription": [{"value": "Product based on polyurethane or silane modified polymer, group 2 (of product based on polyurethane or silane modified polymer, group 2)", "lang": "en"}], "type": "flow data set", "refObjectId": "d14a35d7-b407-b599-93ab-25a0d0dc8c33", "uri": "../flows/d14a35d7-b407-b599-93ab-25a0d0dc8c33.xml"}, "meanAmount": 1.0, "referencesToDataSource": {}, "referenceFlow": true, "resolvedFlowVersion": "00.02.000", "resultingflowAmount": 1.0, "flowProperties": [{"name": [{"lang": "en", "value": "Mass"}, {"lang": "de", "value": "Masse"}], "uuid": "93a60a56-a3c8-11da-a746-0800200b9a66", "referenceFlowProperty": true, "meanValue": 1.0, "referenceUnit": "kg", "unitGroupUUID": "ad38d542-3fe9-439d-9b95-2f5f7752acaf"}], "typeOfFlow": "Product flow", "classification": {"classHierarchy": "Beschichtungen / Reaktionsharze / Reaktionsharze auf PU-Basis", "name": "OEKOBAU.DAT"}}, {"dataSetInternalID": 1, "referenceToFlowDataSet": {"shortDescription": [{"value": "Renewable primary energy as energy carrier (PERE)", "lang": "en"}, {"value": "Erneuerbare Primärenergie als Energieträger (PERE)", "lang": "de"}], "type": "flow data set", "refObjectId": "20f32be5-0398-4288-9b6d-accddd195317", "uri": "../flows/20f32be5-0398-4288-9b6d-accddd195317.xml"}, "exchange direction": "INPUT", "other": {"anies": [{"name": "referenceToUnitGroupDataSet", "value": {"shortDescription": [{"value": "MJ", "lang": "en"}], "type": "unit group data set", "refObjectId": "93a60a57-a3c8-11da-a746-0800200c9a66", "uri": "../unitgroups/93a60a57-a3c8-11da-a746-0800200c9a66.xml"}}, {"value": "9.46429", "module": "A1-A3"}, {"value": "0.039", "module": "A4"}, {"value": "0.693", "module": "A5"}, {"value": "1.2E-05", "module": "C1"}, {"value": "0.000525", "module": "C2"}, {"value": "0.0823", "module": "C3"}, {"value": "-3.52", "module": "D"}]}, "resolvedFlowVersion": "38.00.000", "flowProperties": [], "typeOfFlow": "Other flow", "classification": {"classHierarchy": "Quantities", "name": "GaBiCategories"}}, {"dataSetInternalID": 2, "referenceToFlowDataSet": {"shortDescription": [{"value": "Renewable primary energy resources as material utilization (PERM)", "lang": "en"}, {"value": "Erneuerbare Primärenergie zur stofflichen Nutzung (PERM)", "lang": "de"}], "type": "flow data set", "refObjectId": "fb3ec0de-548d-4508-aea5-00b73bf6f702", "uri": "../flows/fb3ec0de-548d-4508-aea5-00b73bf6f702.xml"}, "exchange direction": "INPUT", "other": {"anies": [{"name": "referenceToUnitGroupDataSet", "value": {"shortDescription": [{"value": "MJ", "lang": "en"}], "type": "unit group data set", "refObjectId": "93a60a57-a3c8-11da-a746-0800200c9a66", "uri": "../unitgroups/93a60a57-a3c8-11da-a746-0800200c9a66.xml"}}, {"value": "0.585", "module": "A1-A3"}, {"value": "0", "module": "A4"}, {"value": "-0.585", "module": "A5"}, {"value": "0", "module": "C1"}, {"value": "0", "module": "C2"}, {"value": "0", "module": "C3"}, {"value": "0", "module": "D"}]}, "resolvedFlowVersion": "38.00.000", "flowProperties": [], "typeOfFlow": "Other flow", "classification": {"classHierarchy": "Quantities", "name": "GaBiCategories"}}, {"dataSetInternalID": 3, "referenceToFlowDataSet": {"shortDescription": [{"value": "Total use of renewable primary energy resources (PERT)", "lang": "en"}, {"value": "Total erneuerbare Primärenergie (PERT)", "lang": "de"}], "type": "flow data set", "refObjectId": "53f97275-fa8a-4cdd-9024-65936002acd0", "uri": "../flows/53f97275-fa8a-4cdd-9024-65936002acd0.xml"}, "exchange direction": "INPUT", "other": {"anies": [{"name": "referenceToUnitGroupDataSet", "value": {"shortDescription": [{"value": "MJ", "lang": "en"}], "type": "unit group data set", "refObjectId": "93a60a57-a3c8-11da-a746-0800200c9a66", "uri": "../unitgroups/93a60a57-a3c8-11da-a746-0800200c9a66.xml"}}, {"value": "10.05429", "module": "A1-A3"}, {"value": "0.039", "module": "A4"}, {"value": "0.108", "module": "A5"}, {"value": "1.2E-05", "module": "C1"}, {"value": "0.000525", "module": "C2"}, {"value": "0.0823", "module": "C3"}, {"value": "-3.52", "module": "D"}]}, "resolvedFlowVersion": "38.00.000", "flowProperties": [], "typeOfFlow": "Other flow", "classification": {"classHierarchy": "Quantities / Environmental quantities / EPD EN 15804 / LCI indicators", "name": "GaBiCategories"}}, {"dataSetInternalID": 4, "referenceToFlowDataSet": {"shortDescription": [{"value": "Non renewable primary energy as energy carrier (PENRE)", "lang": "en"}, {"value": "Nicht-erneuerbare Primärenergie als Energieträger (PENRE)", "lang": "de"}], "type": "flow data set", "refObjectId": "ac857178-2b45-46ec-892a-a9a4332f0372", "uri": "../flows/ac857178-2b45-46ec-892a-a9a4332f0372.xml"}, "exchange direction": "INPUT", "other": {"anies": [{"name": "referenceToUnitGroupDataSet", "value": {"shortDescription": [{"value": "MJ", "lang": "en"}], "type": "unit group data set", "refObjectId": "93a60a57-a3c8-11da-a746-0800200c9a66", "uri": "../unitgroups/93a60a57-a3c8-11da-a746-0800200c9a66.xml"}}, {"value": "141.76", "module": "A1-A3"}, {"value": "0.695", "module": "A4"}, {"value": "2.25", "module": "A5"}, {"value": "0.00381", "module": "C1"}, {"value": "0.167", "module": "C2"}, {"value": "25.6", "module": "C3"}, {"value": "-16.1", "module": "D"}]}, "resolvedFlowVersion": "38.00.000", "flowProperties": [], "typeOfFlow": "Other flow", "classification": {"classHierarchy": "Quantities", "name": "GaBiCategories"}}, {"dataSetInternalID": 5, "referenceToFlowDataSet": {"shortDescription": [{"value": "Non renewable primary energy as material utilization (PENRM)", "lang": "en"}, {"value": "Nicht-erneuerbare Primärenergie zur stofflichen Nutzung (PENRM)", "lang": "de"}], "type": "flow data set", "refObjectId": "1421caa0-679d-4bf4-b282-0eb850ccae27", "uri": "../flows/1421caa0-679d-4bf4-b282-0eb850ccae27.xml"}, "exchange direction": "INPUT", "other": {"anies": [{"name": "referenceToUnitGroupDataSet", "value": {"shortDescription": [{"value": "MJ", "lang": "en"}], "type": "unit group data set", "refObjectId": "93a60a57-a3c8-11da-a746-0800200c9a66", "uri": "../unitgroups/93a60a57-a3c8-11da-a746-0800200c9a66.xml"}}, {"value": "25.5", "module": "A1-A3"}, {"value": "0", "module": "A4"}, {"value": "-0.52", "module": "A5"}, {"value": "0", "module": "C1"}, {"value": "0", "module": "C2"}, {"value": "-25", "module": "C3"}, {"value": "0", "module": "D"}]}, "resolvedFlowVersion": "38.00.000", "flowProperties": [], "typeOfFlow": "Other flow", "classification": {"classHierarchy": "Quantities", "name": "GaBiCategories"}}, {"dataSetInternalID": 6, "referenceToFlowDataSet": {"shortDescription": [{"value": "Total use of non renewable primary energy resources (PENRT)", "lang": "en"}, {"value": "Total nicht erneuerbare Primärenergie (PENRT)", "lang": "de"}], "type": "flow data set", "refObjectId": "06159210-646b-4c8d-8583-da9b3b95a6c1", "uri": "../flows/06159210-646b-4c8d-8583-da9b3b95a6c1.xml"}, "exchange direction": "INPUT", "other": {"anies": [{"name": "referenceToUnitGroupDataSet", "value": {"shortDescription": [{"value": "MJ", "lang": "en"}], "type": "unit group data set", "refObjectId": "93a60a57-a3c8-11da-a746-0800200c9a66", "uri": "../unitgroups/93a60a57-a3c8-11da-a746-0800200c9a66.xml"}}, {"value": "167.32", "module": "A1-A3"}, {"value": "0.695", "module": "A4"}, {"value": "1.73", "module": "A5"}, {"value": "0.00381", "module": "C1"}, {"value": "0.167", "module": "C2"}, {"value": "0.587", "module": "C3"}, {"value": "-16.1", "module": "D"}]}, "resolvedFlowVersion": "38.00.000", "flowProperties": [], "typeOfFlow": "Other flow", "classification": {"classHierarchy": "Quantities / Environmental quantities / EPD EN 15804 / LCI indicators", "name": "GaBiCategories"}}, {"dataSetInternalID": 7, "referenceToFlowDataSet": {"shortDescription": [{"value": "Use of secondary material (SM)", "lang": "en"}, {"value": "Einsatz von Sekundärstoffen (SM)", "lang": "de"}], "type": "flow data set", "refObjectId": "c6a1f35f-2d09-4f54-8dfb-97e502e1ce92", "uri": "../flows/c6a1f35f-2d09-4f54-8dfb-97e502e1ce92.xml"}, "exchange direction": "INPUT", "other": {"anies": [{"name": "referenceToUnitGroupDataSet", "value": {"shortDescription": [{"value": "kg", "lang": "en"}], "type": "unit group data set", "refObjectId": "ad38d542-3fe9-439d-9b95-2f5f7752acaf", "uri": "../unitgroups/ad38d542-3fe9-439d-9b95-2f5f7752acaf.xml"}}, {"value": "0", "module": "A1-A3"}, {"value": "0", "module": "A4"}, {"value": "0", "module": "A5"}, {"value": "0", "module": "C1"}, {"value": "0", "module": "C2"}, {"value": "0", "module": "C3"}, {"value": "0", "module": "D"}]}, "resolvedFlowVersion": "38.00.000", "flowProperties": [], "typeOfFlow": "Other flow", "classification": {"classHierarchy": "Quantities / Environmental quantities / EPD EN 15804 / LCI indicators", "name": "GaBiCategories"}}, {"dataSetInternalID": 8, "referenceToFlowDataSet": {"shortDescription": [{"value": "Use of renewable secondary fuels (RSF)", "lang": "en"}, {"value": "Erneuerbare Sekundärbrennstoffe (RSF)", "lang": "de"}], "type": "flow data set", "refObjectId": "64333088-a55f-4aa2-9a31-c10b07816787", "uri": "../flows/64333088-a55f-4aa2-9a31-c10b07816787.xml"}, "exchange direction": "INPUT", "other": {"anies": [{"name": "referenceToUnitGroupDataSet", "value": {"shortDescription": [{"value": "MJ", "lang": "en"}], "type": "unit group data set", "refObjectId": "93a60a57-a3c8-11da-a746-0800200c9a66", "uri": "../unitgroups/93a60a57-a3c8-11da-a746-0800200c9a66.xml"}}, {"value": "0", "module": "A1-A3"}, {"value": "0", "module": "A4"}, {"value": "0", "module": "A5"}, {"value": "0", "module": "C1"}, {"value": "0", "module": "C2"}, {"value": "0", "module": "C3"}, {"value": "0", "module": "D"}]}, "resolvedFlowVersion": "38.00.000", "flowProperties": [], "typeOfFlow": "Other flow", "classification": {"classHierarchy": "Quantities / Environmental quantities / EPD EN 15804 / LCI indicators", "name": "GaBiCategories"}}, {"dataSetInternalID": 9, "referenceToFlowDataSet": {"shortDescription": [{"value": "Use of non renewable secondary fuels (NRSF)", "lang": "en"}, {"value": "Nicht erneuerbare Sekundärbrennstoffe (NRSF)", "lang": "de"}], "type": "flow data set", "refObjectId": "89def144-d39a-4287-b86f-efde453ddcb2", "uri": "../flows/89def144-d39a-4287-b86f-efde453ddcb2.xml"}, "exchange direction": "INPUT", "other": {"anies": [{"name": "referenceToUnitGroupDataSet", "value": {"shortDescription": [{"value": "MJ", "lang": "en"}], "type": "unit group data set", "refObjectId": "93a60a57-a3c8-11da-a746-0800200c9a66", "uri": "../unitgroups/93a60a57-a3c8-11da-a746-0800200c9a66.xml"}}, {"value": "0", "module": "A1-A3"}, {"value": "0", "module": "A4"}, {"value": "0", "module": "A5"}, {"value": "0", "module": "C1"}, {"value": "0", "module": "C2"}, {"value": "0", "module": "C3"}, {"value": "0", "module": "D"}]}, "resolvedFlowVersion": "38.00.000", "flowProperties": [], "typeOfFlow": "Other flow", "classification": {"classHierarchy": "Quantities / Environmental quantities / EPD EN 15804 / LCI indicators", "name": "GaBiCategories"}}, {"dataSetInternalID": 10, "referenceToFlowDataSet": {"shortDescription": [{"value": "Use of net fresh water (FW)", "lang": "en"}, {"value": "Einsatz von Süßwasserressourcen (FW)", "lang": "de"}], "type": "flow data set", "refObjectId": "3cf952c8-f3a4-461d-8c96-96456ca62246", "uri": "../flows/3cf952c8-f3a4-461d-8c96-96456ca62246.xml"}, "exchange direction": "INPUT", "other": {"anies": [{"name": "referenceToUnitGroupDataSet", "value": {"shortDescription": [{"value": "m^3", "lang": "en"}], "type": "unit group data set", "refObjectId": "cd950537-0a98-4044-9ba7-9f9a68d0a504", "uri": "../unitgroups/cd950537-0a98-4044-9ba7-9f9a68d0a504.xml"}}, {"value": "0.03549569", "module": "A1-A3"}, {"value": "4.52E-05", "module": "A4"}, {"value": "0.000675", "module": "A5"}, {"value": "2.16E-08", "module": "C1"}, {"value": "9.41E-07", "module": "C2"}, {"value": "0.00511", "module": "C3"}, {"value": "-0.00408", "module": "D"}]}, "resolvedFlowVersion": "38.00.000", "flowProperties": [], "typeOfFlow": "Other flow", "classification": {"classHierarchy": "Quantities / Environmental quantities / EPD EN 15804 / LCI indicators", "name": "GaBiCategories"}}, {"dataSetInternalID": 11, "referenceToFlowDataSet": {"shortDescription": [{"value": "Hazardous waste disposed (HWD)", "lang": "en"}, {"value": "Gefährlicher Abfall zur Deponie (HWD)", "lang": "de"}], "type": "flow data set", "refObjectId": "430f9e0f-59b2-46a0-8e0d-55e0e84948fc", "uri": "../flows/430f9e0f-59b2-46a0-8e0d-55e0e84948fc.xml"}, "exchange direction": "OUTPUT", "other": {"anies": [{"name": "referenceToUnitGroupDataSet", "value": {"shortDescription": [{"value": "kg", "lang": "en"}], "type": "unit group data set", "refObjectId": "ad38d542-3fe9-439d-9b95-2f5f7752acaf", "uri": "../unitgroups/ad38d542-3fe9-439d-9b95-2f5f7752acaf.xml"}}, {"value": "4.3542E-08", "module": "A1-A3"}, {"value": "3.23E-08", "module": "A4"}, {"value": "6.08E-10", "module": "A5"}, {"value": "3.7E-13", "module": "C1"}, {"value": "1.62E-11", "module": "C2"}, {"value": "3.34E-10", "module": "C3"}, {"value": "-6.41E-09", "module": "D"}]}, "resolvedFlowVersion": "38.00.000", "flowProperties": [], "typeOfFlow": "Other flow", "classification": {"classHierarchy": "Quantities / Environmental quantities / EPD EN 15804 / LCI indicators", "name": "GaBiCategories"}}, {"dataSetInternalID": 12, "referenceToFlowDataSet": {"shortDescription": [{"value": "Non hazardous waste disposed (NHWD)", "lang": "en"}, {"value": "Entsorgter nicht gefährlicher Abfall (NHWD)", "lang": "de"}], "type": "flow data set", "refObjectId": "b29ef66b-e286-4afa-949f-62f1a7b4d7fa", "uri": "../flows/b29ef66b-e286-4afa-949f-62f1a7b4d7fa.xml"}, "exchange direction": "OUTPUT", "other": {"anies": [{"name": "referenceToUnitGroupDataSet", "value": {"shortDescription": [{"value": "kg", "lang": "en"}], "type": "unit group data set", "refObjectId": "ad38d542-3fe9-439d-9b95-2f5f7752acaf", "uri": "../unitgroups/ad38d542-3fe9-439d-9b95-2f5f7752acaf.xml"}}, {"value": "0.317149", "module": "A1-A3"}, {"value": "0.000106", "module": "A4"}, {"value": "0.049", "module": "A5"}, {"value": "3.9E-07", "module": "C1"}, {"value": "1.7E-05", "module": "C2"}, {"value": "0.0111", "module": "C3"}, {"value": "-0.00744", "module": "D"}]}, "resolvedFlowVersion": "38.00.000", "flowProperties": [], "typeOfFlow": "Other flow", "classification": {"classHierarchy": "Quantities / Environmental quantities / EPD EN 15804 / LCI indicators", "name": "GaBiCategories"}}, {"dataSetInternalID": 13, "referenceToFlowDataSet": {"shortDescription": [{"value": "Radioactive waste disposed (RWD)", "lang": "en"}, {"value": "Entsorgter radioaktiver Abfall (RWD)", "lang": "de"}], "type": "flow data set", "refObjectId": "3449546e-52ad-4b39-b809-9fb77cea8ff6", "uri": "../flows/3449546e-52ad-4b39-b809-9fb77cea8ff6.xml"}, "exchange direction": "OUTPUT", "other": {"anies": [{"name": "referenceToUnitGroupDataSet", "value": {"shortDescription": [{"value": "kg", "lang": "en"}], "type": "unit group data set", "refObjectId": "ad38d542-3fe9-439d-9b95-2f5f7752acaf", "uri": "../unitgroups/ad38d542-3fe9-439d-9b95-2f5f7752acaf.xml"}}, {"value": "0.00305146", "module": "A1-A3"}, {"value": "8.6E-07", "module": "A4"}, {"value": "3.24E-05", "module": "A5"}, {"value": "4.09E-09", "module": "C1"}, {"value": "1.79E-07", "module": "C2"}, {"value": "2.37E-05", "module": "C3"}, {"value": "-0.0012", "module": "D"}]}, "resolvedFlowVersion": "38.00.000", "flowProperties": [], "typeOfFlow": "Other flow", "classification": {"classHierarchy": "Quantities / Environmental quantities / EPD EN 15804 / LCI indicators", "name": "GaBiCategories"}}, {"dataSetInternalID": 14, "referenceToFlowDataSet": {"shortDescription": [{"value": "Components for re-use (CRU)", "lang": "en"}, {"value": "Komponenten für die Wiederverwendung (CRU)", "lang": "de"}], "type": "flow data set", "refObjectId": "a2b32f97-3fc7-4af2-b209-525bc6426f33", "uri": "../flows/a2b32f97-3fc7-4af2-b209-525bc6426f33.xml"}, "exchange direction": "OUTPUT", "other": {"anies": [{"name": "referenceToUnitGroupDataSet", "value": {"shortDescription": [{"value": "kg", "lang": "en"}], "type": "unit group data set", "refObjectId": "ad38d542-3fe9-439d-9b95-2f5f7752acaf", "uri": "../unitgroups/ad38d542-3fe9-439d-9b95-2f5f7752acaf.xml"}}, {"value": "0", "module": "A1-A3"}, {"value": "0", "module": "A4"}, {"value": "0", "module": "A5"}, {"value": "0", "module": "C1"}, {"value": "0", "module": "C2"}, {"value": "0", "module": "C3"}, {"value": "0", "module": "D"}]}, "resolvedFlowVersion": "38.00.000", "flowProperties": [], "typeOfFlow": "Other flow", "classification": {"classHierarchy": "Quantities / Environmental quantities / EPD EN 15804 / LCI indicators", "name": "GaBiCategories"}}, {"dataSetInternalID": 15, "referenceToFlowDataSet": {"shortDescription": [{"value": "Materials for recycling (MFR)", "lang": "en"}, {"value": "Stoffe zum Recycling (MFR)", "lang": "de"}], "type": "flow data set", "refObjectId": "d7fe48a5-4103-49c8-9aae-b0b5dfdbd6ae", "uri": "../flows/d7fe48a5-4103-49c8-9aae-b0b5dfdbd6ae.xml"}, "exchange direction": "OUTPUT", "other": {"anies": [{"name": "referenceToUnitGroupDataSet", "value": {"shortDescription": [{"value": "kg", "lang": "en"}], "type": "unit group data set", "refObjectId": "ad38d542-3fe9-439d-9b95-2f5f7752acaf", "uri": "../unitgroups/ad38d542-3fe9-439d-9b95-2f5f7752acaf.xml"}}, {"value": "0", "module": "A1-A3"}, {"value": "0", "module": "A4"}, {"value": "0", "module": "A5"}, {"value": "0", "module": "C1"}, {"value": "0", "module": "C2"}, {"value": "0", "module": "C3"}, {"value": "0", "module": "D"}]}, "resolvedFlowVersion": "38.00.000", "flowProperties": [], "typeOfFlow": "Other flow", "classification": {"classHierarchy": "Quantities / Environmental quantities / EPD EN 15804 / LCI indicators", "name": "GaBiCategories"}}, {"dataSetInternalID": 16, "referenceToFlowDataSet": {"shortDescription": [{"value": "Materials for energy recovery (MER)", "lang": "en"}, {"value": "Stoffe für die Energierückgewinnung (MER)", "lang": "de"}], "type": "flow data set", "refObjectId": "59a9181c-3aaf-46ee-8b13-2b3723b6e447", "uri": "../flows/59a9181c-3aaf-46ee-8b13-2b3723b6e447.xml"}, "exchange direction": "OUTPUT", "other": {"anies": [{"name": "referenceToUnitGroupDataSet", "value": {"shortDescription": [{"value": "kg", "lang": "en"}], "type": "unit group data set", "refObjectId": "ad38d542-3fe9-439d-9b95-2f5f7752acaf", "uri": "../unitgroups/ad38d542-3fe9-439d-9b95-2f5f7752acaf.xml"}}, {"value": "0", "module": "A1-A3"}, {"value": "0", "module": "A4"}, {"value": "0", "module": "A5"}, {"value": "0", "module": "C1"}, {"value": "0", "module": "C2"}, {"value": "0", "module": "C3"}, {"value": "0", "module": "D"}]}, "resolvedFlowVersion": "38.00.000", "flowProperties": [], "typeOfFlow": "Other flow", "classification": {"classHierarchy": "Quantities / Environmental quantities / EPD EN 15804 / LCI indicators", "name": "GaBiCategories"}}, {"dataSetInternalID": 17, "referenceToFlowDataSet": {"shortDescription": [{"value": "Exported electrical energy (EEE)", "lang": "en"}, {"value": "Exportierte elektrische Energie (EEE)", "lang": "de"}], "type": "flow data set", "refObjectId": "4da0c987-2b76-40d6-9e9e-82a017aaaf29", "uri": "../flows/4da0c987-2b76-40d6-9e9e-82a017aaaf29.xml"}, "exchange direction": "OUTPUT", "other": {"anies": [{"name": "referenceToUnitGroupDataSet", "value": {"shortDescription": [{"value": "MJ", "lang": "en"}], "type": "unit group data set", "refObjectId": "93a60a57-a3c8-11da-a746-0800200c9a66", "uri": "../unitgroups/93a60a57-a3c8-11da-a746-0800200c9a66.xml"}}, {"value": "0", "module": "A1-A3"}, {"value": "0", "module": "A4"}, {"value": "0.212", "module": "A5"}, {"value": "0", "module": "C1"}, {"value": "0", "module": "C2"}, {"value": "0", "module": "C3"}, {"value": "0", "module": "D"}]}, "resolvedFlowVersion": "38.00.000", "flowProperties": [], "typeOfFlow": "Other flow", "classification": {"classHierarchy": "Quantities / Environmental quantities / EPD EN 15804 / LCI indicators", "name": "GaBiCategories"}}, {"dataSetInternalID": 18, "referenceToFlowDataSet": {"shortDescription": [{"value": "Exported thermal energy (EET)", "lang": "en"}, {"value": "Exportierte thermische Energie (EET)", "lang": "de"}], "type": "flow data set", "refObjectId": "98daf38a-7a79-46d3-9a37-2b7bd0955810", "uri": "../flows/98daf38a-7a79-46d3-9a37-2b7bd0955810.xml"}, "exchange direction": "OUTPUT", "other": {"anies": [{"name": "referenceToUnitGroupDataSet", "value": {"shortDescription": [{"value": "MJ", "lang": "en"}], "type": "unit group data set", "refObjectId": "93a60a57-a3c8-11da-a746-0800200c9a66", "uri": "../unitgroups/93a60a57-a3c8-11da-a746-0800200c9a66.xml"}}, {"value": "0", "module": "A1-A3"}, {"value": "0", "module": "A4"}, {"value": "0.386", "module": "A5"}, {"value": "0", "module": "C1"}, {"value": "0", "module": "C2"}, {"value": "0", "module": "C3"}, {"value": "0", "module": "D"}]}, "resolvedFlowVersion": "38.00.000", "flowProperties": [], "typeOfFlow": "Other flow", "classification": {"classHierarchy": "Quantities / Environmental quantities / EPD EN 15804 / LCI indicators", "name": "GaBiCategories"}}]}, "LCIAResults": {"LCIAResult": [{"referenceToLCIAMethodDataSet": {"shortDescription": [{"value": "Global Warming Potential total (GWP-total)", "lang": "en"}, {"value": "Globales Erwärmungspotenzial total (GWP-total)", "lang": "de"}], "type": "LCIA method data set", "refObjectId": "6a37f984-a4b3-458a-a20a-64418c145fa2", "uri": "../lciamethods/6a37f984-a4b3-458a-a20a-64418c145fa2.xml"}, "other": {"anies": [{"name": "referenceToUnitGroupDataSet", "value": {"shortDescription": [{"value": "kg CO_(2)-Äq.", "lang": "en"}], "type": "unit group data set", "refObjectId": "1ebf3012-d0db-4de2-aefd-ef30cedb0be1", "uri": "../unitgroups/1ebf3012-d0db-4de2-aefd-ef30cedb0be1.xml"}}, {"value": "8.045", "module": "A1-A3"}, {"value": "0.0527", "module": "A4"}, {"value": "0.213", "module": "A5"}, {"value": "0.000279", "module": "C1"}, {"value": "0.0124", "module": "C2"}, {"value": "2.21", "module": "C3"}, {"value": "-0.95", "module": "D"}]}}, {"referenceToLCIAMethodDataSet": {"shortDescription": [{"value": "Global Warming Potential fossil fuels (GWP-fossil)", "lang": "en"}, {"value": "Globales Erwärmungspotenzial fossil (GWP-fossil)", "lang": "de"}], "type": "LCIA method data set", "refObjectId": "5f635281-343e-44fb-83df-1971b155e6b6", "uri": "../lciamethods/5f635281-343e-44fb-83df-1971b155e6b6.xml"}, "other": {"anies": [{"name": "referenceToUnitGroupDataSet", "value": {"shortDescription": [{"value": "kg CO_(2)-Äq.", "lang": "en"}], "type": "unit group data set", "refObjectId": "1ebf3012-d0db-4de2-aefd-ef30cedb0be1", "uri": "../unitgroups/1ebf3012-d0db-4de2-aefd-ef30cedb0be1.xml"}}, {"value": "7.8885", "module": "A1-A3"}, {"value": "0.0522", "module": "A4"}, {"value": "0.125", "module": "A5"}, {"value": "0.000266", "module": "C1"}, {"value": "0.0118", "module": "C2"}, {"value": "2.21", "module": "C3"}, {"value": "-0.947", "module": "D"}]}}, {"referenceToLCIAMethodDataSet": {"shortDescription": [{"value": "Global Warming Potential biogenic (GWP-biogenic)", "lang": "en"}, {"value": "Globales Erwärmungspotenzial biogen (GWP-biogenic)", "lang": "de"}], "type": "LCIA method data set", "refObjectId": "2356e1ab-0185-4db5-86e5-16de51c7485c", "uri": "../lciamethods/2356e1ab-0185-4db5-86e5-16de51c7485c.xml"}, "other": {"anies": [{"name": "referenceToUnitGroupDataSet", "value": {"shortDescription": [{"value": "kg CO_(2)-Äq.", "lang": "en"}], "type": "unit group data set", "refObjectId": "1ebf3012-d0db-4de2-aefd-ef30cedb0be1", "uri": "../unitgroups/1ebf3012-d0db-4de2-aefd-ef30cedb0be1.xml"}}, {"value": "0.15033", "module": "A1-A3"}, {"value": "0.000152", "module": "A4"}, {"value": "0.0881", "module": "A5"}, {"value": "1.24E-05", "module": "C1"}, {"value": "0.000542", "module": "C2"}, {"value": "8.82E-05", "module": "C3"}, {"value": "-0.00223", "module": "D"}]}}, {"referenceToLCIAMethodDataSet": {"shortDescription": [{"value": "Global Warming Potential luluc (GWP-luluc)", "lang": "en"}, {"value": "Globales Erwärmungspotenzial luluc (GWP-luluc)", "lang": "de"}], "type": "LCIA method data set", "refObjectId": "4331bbdb-978a-490d-8707-eeb047f01a55", "uri": "../lciamethods/4331bbdb-978a-490d-8707-eeb047f01a55.xml"}, "other": {"anies": [{"name": "referenceToUnitGroupDataSet", "value": {"shortDescription": [{"value": "kg CO_(2)-Äq.", "lang": "en"}], "type": "unit group data set", "refObjectId": "1ebf3012-d0db-4de2-aefd-ef30cedb0be1", "uri": "../unitgroups/1ebf3012-d0db-4de2-aefd-ef30cedb0be1.xml"}}, {"value": "0.00216628", "module": "A1-A3"}, {"value": "0.000422", "module": "A4"}, {"value": "2.51E-05", "module": "A5"}, {"value": "6.39E-09", "module": "C1"}, {"value": "2.79E-07", "module": "C2"}, {"value": "2.08E-05", "module": "C3"}, {"value": "-0.000666", "module": "D"}]}}, {"referenceToLCIAMethodDataSet": {"shortDescription": [{"value": "Depletion potential of the stratospheric ozone layer (ODP)", "lang": "en"}, {"value": "Abbau Potential der stratosphärischen Ozonschicht (ODP)", "lang": "de"}], "type": "LCIA method data set", "refObjectId": "b5c629d6-def3-11e6-bf01-fe55135034f3", "uri": "../lciamethods/b5c629d6-def3-11e6-bf01-fe55135034f3.xml"}, "other": {"anies": [{"name": "referenceToUnitGroupDataSet", "value": {"shortDescription": [{"value": "kg CFC11-Äq.", "lang": "en"}], "type": "unit group data set", "refObjectId": "d9e957c9-7309-4474-bf3a-7777df6c4e5b", "uri": "../unitgroups/d9e957c9-7309-4474-bf3a-7777df6c4e5b.xml"}}, {"value": "2.7400014501E-09", "module": "A1-A3"}, {"value": "6.27E-18", "module": "A4"}, {"value": "2.74E-11", "module": "A5"}, {"value": "2.84E-20", "module": "C1"}, {"value": "1.24E-18", "module": "C2"}, {"value": "2.62E-16", "module": "C3"}, {"value": "-9.93E-15", "module": "D"}]}}, {"referenceToLCIAMethodDataSet": {"shortDescription": [{"value": "Acidification potential of land and water (AP)", "lang": "en"}, {"value": "Versauerungspotenzial von Boden und Wasser (AP)", "lang": "de"}], "type": "LCIA method data set", "refObjectId": "b5c611c6-def3-11e6-bf01-fe55135034f3", "uri": "../lciamethods/b5c611c6-def3-11e6-bf01-fe55135034f3.xml"}, "other": {"anies": [{"name": "referenceToUnitGroupDataSet", "value": {"shortDescription": [{"value": "mol H^(+)-Äq.", "lang": "en"}], "type": "unit group data set", "refObjectId": "42e089ac-92bf-4bf2-8ca1-5fc40d18f2ed", "uri": "../unitgroups/42e089ac-92bf-4bf2-8ca1-5fc40d18f2ed.xml"}}, {"value": "0.014772", "module": "A1-A3"}, {"value": "0.000156", "module": "A4"}, {"value": "0.000176", "module": "A5"}, {"value": "3.6E-06", "module": "C1"}, {"value": "3.73E-05", "module": "C2"}, {"value": "0.00131", "module": "C3"}, {"value": "-0.00133", "module": "D"}]}}, {"referenceToLCIAMethodDataSet": {"shortDescription": [{"value": "Eutrophication potential aquatic freshwater (EP-freshwater)", "lang": "en"}, {"value": "Eutrophierungspotenzial Süßwasser (EP-freshwater)", "lang": "de"}], "type": "LCIA method data set", "refObjectId": "b53ec18f-7377-4ad3-86eb-cc3f4f276b2b", "uri": "../lciamethods/b53ec18f-7377-4ad3-86eb-cc3f4f276b2b.xml"}, "other": {"anies": [{"name": "referenceToUnitGroupDataSet", "value": {"shortDescription": [{"value": "kg PO_(4)-Äq.", "lang": "en"}], "type": "unit group data set", "refObjectId": "0429039d-a61d-4590-ba67-aa4a20a810a1", "uri": "../unitgroups/0429039d-a61d-4590-ba67-aa4a20a810a1.xml"}}, {"value": "1.30475E-05", "module": "A1-A3"}, {"value": "1.59E-07", "module": "A4"}, {"value": "1.35E-07", "module": "A5"}, {"value": "5.75E-11", "module": "C1"}, {"value": "2.51E-09", "module": "C2"}, {"value": "4.4E-08", "module": "C3"}, {"value": "-1.23E-06", "module": "D"}]}}, {"referenceToLCIAMethodDataSet": {"shortDescription": [{"value": "Eutrophication potential aquatic marine (EP-marine)", "lang": "en"}, {"value": "Eutrophierungspotenzial Salzwasser (EP-marine)", "lang": "de"}], "type": "LCIA method data set", "refObjectId": "b5c619fa-def3-11e6-bf01-fe55135034f3", "uri": "../lciamethods/b5c619fa-def3-11e6-bf01-fe55135034f3.xml"}, "other": {"anies": [{"name": "referenceToUnitGroupDataSet", "value": {"shortDescription": [{"value": "kg N-Äq.", "lang": "en"}], "type": "unit group data set", "refObjectId": "d05bb823-ecdf-4686-8c40-bf1d9257859f", "uri": "../unitgroups/d05bb823-ecdf-4686-8c40-bf1d9257859f.xml"}}, {"value": "0.004388", "module": "A1-A3"}, {"value": "6.96E-05", "module": "A4"}, {"value": "5.22E-05", "module": "A5"}, {"value": "1.63E-06", "module": "C1"}, {"value": "1.72E-05", "module": "C2"}, {"value": "0.000631", "module": "C3"}, {"value": "-0.000343", "module": "D"}]}}, {"referenceToLCIAMethodDataSet": {"shortDescription": [{"value": "Eutrophication potential terrestrial (EP-terrestrial)", "lang": "en"}, {"value": "Eutrophierungspotenzial Land (EP-terrestrial)", "lang": "de"}], "type": "LCIA method data set", "refObjectId": "b5c614d2-def3-11e6-bf01-fe55135034f3", "uri": "../lciamethods/b5c614d2-def3-11e6-bf01-fe55135034f3.xml"}, "other": {"anies": [{"name": "referenceToUnitGroupDataSet", "value": {"shortDescription": [{"value": "mol N-Äq.", "lang": "en"}], "type": "unit group data set", "refObjectId": "71b4d617-0ec9-4d3f-b65e-e438940c2401", "uri": "../unitgroups/71b4d617-0ec9-4d3f-b65e-e438940c2401.xml"}}, {"value": "0.046", "module": "A1-A3"}, {"value": "0.00078", "module": "A4"}, {"value": "0.000577", "module": "A5"}, {"value": "1.79E-05", "module": "C1"}, {"value": "0.000189", "module": "C2"}, {"value": "0.00726", "module": "C3"}, {"value": "-0.00368", "module": "D"}]}}, {"referenceToLCIAMethodDataSet": {"shortDescription": [{"value": "Formation potential of tropospheric ozone photochemical oxidants (POCP)", "lang": "en"}, {"value": "Bildungspotential für troposphärisches Ozon (POCP)", "lang": "de"}], "type": "LCIA method data set", "refObjectId": "b5c610fe-def3-11e6-bf01-fe55135034f3", "uri": "../lciamethods/b5c610fe-def3-11e6-bf01-fe55135034f3.xml"}, "other": {"anies": [{"name": "referenceToUnitGroupDataSet", "value": {"shortDescription": [{"value": "kg NMVOC-Äq.", "lang": "en"}], "type": "unit group data set", "refObjectId": "d27c25f8-fbc1-44c6-b47b-4adbae4199c6", "uri": "../unitgroups/d27c25f8-fbc1-44c6-b47b-4adbae4199c6.xml"}}, {"value": "0.014853", "module": "A1-A3"}, {"value": "0.000138", "module": "A4"}, {"value": "0.00725", "module": "A5"}, {"value": "4.91E-06", "module": "C1"}, {"value": "3.39E-05", "module": "C2"}, {"value": "0.00162", "module": "C3"}, {"value": "-0.000987", "module": "D"}]}}, {"referenceToLCIAMethodDataSet": {"shortDescription": [{"value": "Abiotic depletion potential for non fossil resources (ADPE)", "lang": "en"}, {"value": "Potenzial für den abiotischen Abbau nicht fossiler Ressourcen (ADPE)", "lang": "de"}], "type": "LCIA method data set", "refObjectId": "b2ad6494-c78d-11e6-9d9d-cec0c932ce01", "uri": "../lciamethods/b2ad6494-c78d-11e6-9d9d-cec0c932ce01.xml"}, "other": {"anies": [{"name": "referenceToUnitGroupDataSet", "value": {"shortDescription": [{"value": "kg Sb-Äq.", "lang": "en"}], "type": "unit group data set", "refObjectId": "54ccd2d9-a32a-4fc2-923d-f2c8c93e89d4", "uri": "../unitgroups/54ccd2d9-a32a-4fc2-923d-f2c8c93e89d4.xml"}}, {"value": "8.35888E-06", "module": "A1-A3"}, {"value": "3.74E-09", "module": "A4"}, {"value": "8.4E-08", "module": "A5"}, {"value": "8.06E-12", "module": "C1"}, {"value": "3.52E-10", "module": "C2"}, {"value": "4.65E-09", "module": "C3"}, {"value": "-1.56E-07", "module": "D"}]}}, {"referenceToLCIAMethodDataSet": {"shortDescription": [{"value": "Abiotic depletion potential for fossil resources (ADPF)", "lang": "en"}, {"value": "Potenzial für den abiotischen Abbau fossiler Brennstoffe (ADPF)", "lang": "de"}], "type": "LCIA method data set", "refObjectId": "b2ad6110-c78d-11e6-9d9d-cec0c932ce01", "uri": "../lciamethods/b2ad6110-c78d-11e6-9d9d-cec0c932ce01.xml"}, "other": {"anies": [{"name": "referenceToUnitGroupDataSet", "value": {"shortDescription": [{"value": "MJ", "lang": "en"}], "type": "unit group data set", "refObjectId": "93a60a57-a3c8-11da-a746-0800200c9a66", "uri": "../unitgroups/93a60a57-a3c8-11da-a746-0800200c9a66.xml"}}, {"value": "166.32", "module": "A1-A3"}, {"value": "0.694", "module": "A4"}, {"value": "1.73", "module": "A5"}, {"value": "0.00381", "module": "C1"}, {"value": "0.166", "module": "C2"}, {"value": "0.587", "module": "C3"}, {"value": "-16.1", "module": "D"}]}}, {"referenceToLCIAMethodDataSet": {"shortDescription": [{"value": "Water use (WDP)", "lang": "en"}, {"value": "Wassernutzung (WDP)", "lang": "de"}], "type": "LCIA method data set", "refObjectId": "b2ad66ce-c78d-11e6-9d9d-cec0c932ce01", "uri": "../lciamethods/b2ad66ce-c78d-11e6-9d9d-cec0c932ce01.xml"}, "other": {"anies": [{"name": "referenceToUnitGroupDataSet", "value": {"shortDescription": [{"value": "m^(3) world-Äq. deprived", "lang": "en"}], "type": "unit group data set", "refObjectId": "6ae2df01-888e-46c8-b17d-49fa3869b476", "uri": "../unitgroups/6ae2df01-888e-46c8-b17d-49fa3869b476.xml"}}, {"value": "1.187588", "module": "A1-A3"}, {"value": "0.000466", "module": "A4"}, {"value": "0.0254", "module": "A5"}, {"value": "5.27E-07", "module": "C1"}, {"value": "2.3E-05", "module": "C2"}, {"value": "0.217", "module": "C3"}, {"value": "-0.0986", "module": "D"}]}}, {"referenceToLCIAMethodDataSet": {"shortDescription": [{"value": "Incidence of disease due to PM emissions (PM)", "lang": "en"}, {"value": "Auftreten von Krankheiten aufgrund von Feinstaubemissionen (PM)", "lang": "de"}], "type": "LCIA method data set", "refObjectId": "b5c602c6-def3-11e6-bf01-fe55135034f3", "uri": "../lciamethods/b5c602c6-def3-11e6-bf01-fe55135034f3.xml"}, "other": {"anies": [{"name": "referenceToUnitGroupDataSet", "value": {"shortDescription": [{"value": "Disease incidence", "lang": "en"}], "type": "unit group data set", "refObjectId": "3883559b-648f-4afc-8ba2-0bd24f3affa3", "uri": "../unitgroups/3883559b-648f-4afc-8ba2-0bd24f3affa3.xml"}}, {"module": "A1-A3"}, {"module": "A4"}, {"module": "A5"}, {"module": "C1"}, {"module": "C2"}, {"module": "C3"}, {"module": "D"}]}}, {"referenceToLCIAMethodDataSet": {"shortDescription": [{"value": "Human exposure efficiency relative to U235 (IR)", "lang": "en"}, {"value": "Wirkung durch Exposition des Menschen mit U235 (IR)", "lang": "de"}], "type": "LCIA method data set", "refObjectId": "b5c632be-def3-11e6-bf01-fe55135034f3", "uri": "../lciamethods/b5c632be-def3-11e6-bf01-fe55135034f3.xml"}, "other": {"anies": [{"name": "referenceToUnitGroupDataSet", "value": {"shortDescription": [{"value": "kBq U235-Äq.", "lang": "en"}], "type": "unit group data set", "refObjectId": "456b05bf-1415-44a9-9993-02452f554c09", "uri": "../unitgroups/456b05bf-1415-44a9-9993-02452f554c09.xml"}}, {"module": "A1-A3"}, {"module": "A4"}, {"module": "A5"}, {"module": "C1"}, {"module": "C2"}, {"module": "C3"}, {"module": "D"}]}}, {"referenceToLCIAMethodDataSet": {"shortDescription": [{"value": "Comparative toxic unit for ecosystems (ETP-fw)", "lang": "en"}, {"value": "Toxizitätsvergleichseinheit für Ökosysteme (ETP-fw)", "lang": "de"}], "type": "LCIA method data set", "refObjectId": "ee1082d1-b0f7-43ca-a1f0-21e2a4a74511", "uri": "../lciamethods/ee1082d1-b0f7-43ca-a1f0-21e2a4a74511.xml"}, "other": {"anies": [{"name": "referenceToUnitGroupDataSet", "value": {"shortDescription": [{"value": "CTUe", "lang": "en"}], "type": "unit group data set", "refObjectId": "aa959ded-f1eb-4efb-9c5c-2d60be36b3e6", "uri": "../unitgroups/aa959ded-f1eb-4efb-9c5c-2d60be36b3e6.xml"}}, {"module": "A1-A3"}, {"module": "A4"}, {"module": "A5"}, {"module": "C1"}, {"module": "C2"}, {"module": "C3"}, {"module": "D"}]}}, {"referenceToLCIAMethodDataSet": {"shortDescription": [{"value": "Comparative toxic unit for humans (carcinogenic) (HTP-c)", "lang": "en"}, {"value": "Toxizitätsvergleichseinheit für Menschen (krebserregend) (HTP-c)", "lang": "de"}], "type": "LCIA method data set", "refObjectId": "2299222a-bbd8-474f-9d4f-4dd1f18aea7c", "uri": "../lciamethods/2299222a-bbd8-474f-9d4f-4dd1f18aea7c.xml"}, "other": {"anies": [{"name": "referenceToUnitGroupDataSet", "value": {"shortDescription": [{"value": "CTUh", "lang": "en"}], "type": "unit group data set", "refObjectId": "d4c9523e-2d7e-49fd-8469-998f547d3a70", "uri": "../unitgroups/d4c9523e-2d7e-49fd-8469-998f547d3a70.xml"}}, {"module": "A1-A3"}, {"module": "A4"}, {"module": "A5"}, {"module": "C1"}, {"module": "C2"}, {"module": "C3"}, {"module": "D"}]}}, {"referenceToLCIAMethodDataSet": {"shortDescription": [{"value": "Comparative toxic unit for humans (noncarcinogenic) (HTP-nc)", "lang": "en"}, {"value": "Toxizitätsvergleichseinheit für Menschen (nicht krebserregend) (HTP-nc)", "lang": "de"}], "type": "LCIA method data set", "refObjectId": "3af763a5-b7a1-48c9-9cee-1f223481fcef", "uri": "../lciamethods/3af763a5-b7a1-48c9-9cee-1f223481fcef.xml"}, "other": {"anies": [{"name": "referenceToUnitGroupDataSet", "value": {"shortDescription": [{"value": "CTUh", "lang": "en"}], "type": "unit group data set", "refObjectId": "d4c9523e-2d7e-49fd-8469-998f547d3a70", "uri": "../unitgroups/d4c9523e-2d7e-49fd-8469-998f547d3a70.xml"}}, {"module": "A1-A3"}, {"module": "A4"}, {"module": "A5"}, {"module": "C1"}, {"module": "C2"}, {"module": "C3"}, {"module": "D"}]}}, {"referenceToLCIAMethodDataSet": {"shortDescription": [{"value": "Soil quality index (SQP)", "lang": "en"}, {"value": "Bodenqualitätsindex (SQP)", "lang": "de"}], "type": "LCIA method data set", "refObjectId": "b2ad6890-c78d-11e6-9d9d-cec0c932ce01", "uri": "../lciamethods/b2ad6890-c78d-11e6-9d9d-cec0c932ce01.xml"}, "other": {"anies": [{"name": "referenceToUnitGroupDataSet", "value": {"shortDescription": [{"value": "SQP", "lang": "en"}], "type": "unit group data set", "refObjectId": "f130951c-e67f-4f7f-8dd4-665de3974e18", "uri": "../unitgroups/f130951c-e67f-4f7f-8dd4-665de3974e18.xml"}}, {"module": "A1-A3"}, {"module": "A4"}, {"module": "A5"}, {"module": "C1"}, {"module": "C2"}, {"module": "C3"}, {"module": "D"}]}}]}, "otherAttributes": {"{http://www.indata.network/EPD/2019}epd-version": "1.2"}, "version": "1.1", "locations": "../ILCDLocations.xml"}