{"processInformation": {"dataSetInformation": {"UUID": "e9be77fc-8a29-40f9-b8f7-105606f279d2", "name": {"baseName": [{"value": "ST PRO Green RC", "lang": "en"}, {"value": "ST PRO Green RC", "lang": "de"}], "functionalUnitFlowProperties": [{"lang": "en"}]}, "classificationInformation": {"classification": [{"class": [{"value": "Komponenten von Fenstern und Vorhangfassaden", "level": 0, "classId": "7"}, {"value": "Rahmen / Profile", "level": 1, "classId": "7.1"}, {"value": "Aluminium", "level": 2, "classId": "7.1.05"}], "name": "OEKOBAU.DAT"}, {"class": [{"value": "02 Building products", "level": 0}, {"value": "Doors, windows, shutters, and related products", "level": 1}, {"value": "Automatic doors, automatic gates, and revolving door systems", "level": 2}], "name": "IBUCategories"}]}, "generalComment": [{"value": "The ST PRO Green RC convinces due to its strengthened profile system and safety. The ST PRO Green RC is tested and certified by ift Rosenheim. A continuous floor rail in the door leaf area and a sabotage protection in the drive prevent the door wings from being levered out.\nAdditional safety is guaranteed due to a multi-point hook locking in the area of the main closing edge.\nThe door variant is equipped with a hook on the secondary closing edge and burglar-resistant glazing.\n\nThe slim profile system can be used with double- and triple glazing, whereby UD values of down to 1.0 W/(m·K) (glass heat transfer coefficient) can be realized.\nTogether with the thermally separated profile the energy losses are minimized\n\nThanks to the new ES PROLINE drive system single door leaves up to 250kg and double door leaves up to 200kg each can be moved quickly and quietly.\n\nThe low energy consumption of the sliding door drive also contributes to the overall energy efficiency of the sliding door system.\nThe drive is suitable for almost all sliding door applications, \n\nincluding use on escape route sliding doors.", "lang": "en"}, {"value": "Der ST PRO Green RC überzeugt durch sein verstärktes Profilsystem und seine Sicherheit. Das ST PRO Green RC ist vom ift Rosenheim geprüft und zertifiziert. Eine durchgehende Bodenschiene im Torblattbereich und ein Sabotageschutz im Antrieb verhindern das Aushebeln der Torflügel. Zusätzliche Sicherheit wird durch eine Mehrpunkt-Hakenverriegelung im Bereich der Hauptschließkante gewährleistet. Die Torvariante ist mit einem Haken an der Nebenschließkante und einer einbruchhemmenden Verglasung ausgestattet. Das schlanke Profilsystem kann mit Zweifach- und Dreifachverglasung eingesetzt werden, wobei UD-Werte von bis zu 1,0 W/(m²-K) (Glaswärmeübergangskoeffizient) realisiert werden können.\nZusammen mit dem thermisch getrennten Profil werden die Energieverluste minimiert. Dank des neuen ES PROLINE-Antriebssystems können Einzeltürflügel bis zu 250 kg und Doppeltürflügel bis zu je 200 kg schnell und leise bewegt werden. Der niedrige Energieverbrauch des Schiebetürantriebs trägt ebenfalls zur Gesamtenergieeffizienz des Schiebetürsystems bei. Der Antrieb eignet sich für fast alle Schiebetüranwendungen, auch für den Einsatz an Fluchtwegschiebetüren.", "lang": "de"}]}, "quantitativeReference": {"referenceToReferenceFlow": [0]}, "time": {"referenceYear": 2021, "dataSetValidUntil": 2026, "other": {"anies": [{"name": "publicationDateOfEPD", "value": 1624838400000}]}}, "geography": {"locationOfOperationSupplyOrProduction": {"location": "DE"}}, "technology": {"technologyDescriptionAndIncludedProcesses": [{"value": "The ST PRO Green RC convinces due to its strengthened profile system and safety. The ST PRO Green RC is tested and certified by ift Rosenheim. A continuous floor rail in the door leaf area and a sabotage protection in the drive prevent the door wings from being levered out. Additional safety is guaranteed due to a multipoint hook locking in the area of the main closing edge. The door variant is equipped with a hook on the secondary closing edge and burglarresistant glazing. \nTechnical data: \nTechnical data of the ES 400 PRO drive system used for ST PRO Green RC standard and emergency exit sliding doors \nDeclared unit: \nThe declared unit is one (1) piece ST PRO Green RC. The declared unit consists of the drive system and two sliding panels. The results for two side screens and a fanlight are presented in the appendix.", "lang": "en"}, {"value": "Der ST PRO Green RC überzeugt durch sein verstärktes Profilsystem und seine Sicherheit. Das ST PRO Green RC ist vom ift Rosenheim geprüft und zertifiziert. Eine durchgehende Bodenschiene im Torblattbereich und ein Sabotageschutz im Antrieb verhindern ein Aushebeln der Torflügel. Zusätzliche Sicherheit wird durch eine Mehrpunkt-Hakenverriegelung im Bereich der Hauptschließkante gewährleistet. Die Türvariante ist mit einem Haken an der Nebenschließkante und einer einbruchhemmenden Verglasung ausgestattet. \nTechnische Daten: \nTechnische Daten des Antriebssystems ES 400 PRO für die Standard- und Notausgangsschiebetüren ST PRO Green RC \nDeklarierte Einheit: \nDie angegebene Einheit ist ein (1) Stück ST PRO Green RC. Die deklarierte Einheit besteht aus dem Antriebssystem und zwei Schiebeflügeln. Die Ergebnisse für zwei Seitenwände und ein Oberlicht finden Sie im Anhang.", "lang": "de"}], "technologicalApplicability": [{"value": "With the ST PRO Green RC sliding door profile system both standard sliding doors and escape route sliding doors can be equipped by using the ES 400 PRO drive system:", "lang": "en"}, {"value": "Mit dem Schiebetürprofilsystem ST PRO Green RC können sowohl Standardschiebetüren als auch Fluchtwegschiebetüren mit dem Antriebssystem ES 400 PRO ausgestattet werden:", "lang": "de"}]}}, "modellingAndValidation": {"LCIMethodAndAllocation": {"typeOfDataSet": "EPD", "referenceToLCAMethodDetails": [{"shortDescription": [{"value": "Automatic doors, automatic gates, and revolving door systems.pdf", "lang": "en"}], "type": "source data set", "refObjectId": "4dbcd047-384c-47a1-922c-209c30c94d53"}], "other": {"anies": [{"name": "subType", "value": "specific dataset"}]}}, "dataSourcesTreatmentAndRepresentativeness": {"referenceToDataSource": [{"shortDescription": [{"value": "GaBi Database (all versions)", "lang": "en"}], "type": "source data set", "refObjectId": "28d74cc0-db8b-4d7e-bc44-5f6d56ce0c4a"}, {"shortDescription": [{"value": "GaBi Database Edition 2020, CUP 2020.02", "lang": "en"}], "type": "source data set", "refObjectId": "4b368ada-d799-4afc-9d41-f371f2b23781"}], "useAdviceForDataSet": [{"value": "Scope: \nThis EPD refers to the entire life cycle of a DORMA ST PRO Green RC automatic sliding door system.\nThe various technical characteristics are outlined in section 2.3. The production location is dormakaba Zusmarshausen, Germany. Product components are also procured from the DORMA facilities in Ennepetal. The material and energy flows were taken into consideration accordingly. \nSystem boundary: \nType of the EPD: cradle to gate - with options\nModules A1-A3, A4, and A5\nThe product stage (A1-A3) begins with considering the production of the necessary raw materials and energies, including all corresponding upstream chains and the actual procurement transports. Furthermore, the entire manufacturing phase was mapped, including the treatment of production waste until the end-of-waste status (EoW) was reached. In addition, both the distribution transports (A4) and the installation including power-consuming tools, installation materials and the packaging waste generated during installation (A5) were taken into account. \n\nModule B6\nModule B6 includes the operational energy use over the Reference Service Life of 15 years.\n\nModules C1-C4\nThe modules include the environmental impacts for dismantling of the ST PRO Green RC and the treatment of the waste categories until end-of-waste status (EoW) is reached, including the associated transports at the end of the product life cycle.\n\nModule D\nIdentification of the benefits and costs of the product outside the system boundary. For plastics, these consist of energy credits from thermal utilization (C3) in the form of the average European electricity mix or thermal energy from natural gas. Recycling of glass and metal scrap results in credits of the respective raw materials.", "lang": "en"}, {"value": "Gültigkeitsbereich: \nDiese EPD bezieht sich auf den gesamten Lebenszyklus eines automatischen Schiebetürsystems DORMA ST PRO Green RC. Die verschiedenen technischen Merkmale werden in Abschnitt 2.3 beschrieben. Der Produktionsstandort ist dormakaba Zusmarshausen, Deutschland. Die Produktkomponenten werden ebenfalls von den DORMA Werken in Ennepetal bezogen. Die Stoff- und Energieströme wurden entsprechend berücksichtigt. \nSystemgrenze: \nArt der EPD: cradle to gate - mit Optionen Module A1-A3, A4 und A5 Die Produktphase (A1-A3) beginnt mit der Betrachtung der Herstellung der benötigten Rohstoffe und Energien, einschließlich aller entsprechenden Vorketten und der eigentlichen Beschaffungstransporte. Außerdem wurde die gesamte Herstellungsphase abgebildet, einschließlich der Behandlung von Produktionsabfällen bis zum Erreichen des End-of-Waste-Status (EoW). Darüber hinaus wurden sowohl die Verteilungstransporte (A4) als auch die Installation einschließlich der stromverbrauchenden Werkzeuge, der Installationsmaterialien und der bei der Installation anfallenden Verpackungsabfälle (A5) berücksichtigt. \n\nModul B6 Modul B6 umfasst den betrieblichen Energieverbrauch über die Referenznutzungsdauer von 15 Jahren. Module C1-C4 Die Module umfassen die Umweltauswirkungen für die Demontage des ST PRO Green RC und die Behandlung der Abfallkategorien bis zum Erreichen des End-of-Waste-Status (EoW), einschließlich der damit verbundenen Transporte am Ende des Produktlebenszyklus. Modul D Identifizierung der Vorteile und Kosten des Produkts außerhalb der Systemgrenze. Bei Kunststoffen bestehen diese aus Energiegutschriften aus der thermischen Verwertung (C3) in Form des durchschnittlichen europäischen Strommixes oder thermischer Energie aus Erdgas. Das Recycling von Glas und Metallschrott führt zu Gutschriften für die entsprechenden Rohstoffe.", "lang": "de"}], "other": {"anies": [{"name": "referenceToOriginalEPD", "value": {"shortDescription": {"value": "ST PRO Green RC.pdf", "defaultValue": "ST PRO Green RC.pdf", "lstrings": [{"lang": "en", "value": "ST PRO Green RC.pdf"}]}, "type": "source data set", "uuid": {"uuid": "3f4d5ae7-0567-4d3a-9cad-1c47cd62e0f6"}, "refObjectId": "3f4d5ae7-0567-4d3a-9cad-1c47cd62e0f6", "resourceURLs": ["https://oekobaudat.de/OEKOBAU.DAT/resource/sources/3f4d5ae7-0567-4d3a-9cad-1c47cd62e0f6/ST_PRO_Green_RC_22576.pdf?version=00.02.000"]}}]}}, "validation": {"review": [{"referenceToNameOfReviewerAndInstitution": [{"shortDescription": [{"value": "Institut Bauen und Umwelt e. V.", "lang": "en"}], "type": "contact data set", "refObjectId": "d111dbec-b024-4be5-86c5-752d6eb2cf95", "uri": "../contacts/d111dbec-b024-4be5-86c5-752d6eb2cf95.xml"}], "type": "Accredited third party review"}]}, "complianceDeclarations": {"compliance": [{"referenceToComplianceSystem": {"shortDescription": [{"value": "DIN EN 15804", "lang": "en"}], "type": "source data set", "refObjectId": "b00f9ec0-7874-11e3-981f-0800200c9a66", "uri": "../sources/b00f9ec0-7874-11e3-981f-0800200c9a66.xml"}}, {"referenceToComplianceSystem": {"shortDescription": [{"value": "ISO 14025", "lang": "en"}], "type": "source data set", "refObjectId": "4f2eb655-6e44-4874-a95a-e28f5442cd4d", "uri": "../sources/4f2eb655-6e44-4874-a95a-e28f5442cd4d.xml"}}]}}, "administrativeInformation": {"commissionerAndGoal": {"referenceToCommissioner": [{"shortDescription": [{"value": "dormakaba International Holding GmbH", "lang": "en"}], "type": "contact data set", "refObjectId": "33313944-7b37-498a-b458-25a295c1017d", "uri": "../contacts/33313944-7b37-498a-b458-25a295c1017d.xml"}]}, "dataGenerator": {"referenceToPersonOrEntityGeneratingTheDataSet": [{"shortDescription": [{"value": "brands and values GmbH", "lang": "en"}], "type": "contact data set", "refObjectId": "6b539b8a-10e3-4004-8ccc-a79f169aa339", "uri": "../contacts/6b539b8a-10e3-4004-8ccc-a79f169aa339.xml"}]}, "dataEntryBy": {"timeStamp": 1624838400000, "referenceToDataSetFormat": [{"shortDescription": [{"value": "ILCD Format", "lang": "en"}], "type": "source data set", "refObjectId": "a97a0155-0234-4b87-b4ce-a45da52f2a40", "uri": "../sources/a97a0155-0234-4b87-b4ce-a45da52f2a40.xml"}, {"shortDescription": [{"value": "EPD-Datenformaterweiterungen v1.2", "lang": "de"}, {"value": "EPD Data Format Extensions v1.2", "lang": "en"}], "type": "source data set", "refObjectId": "a29449fd-aa2f-4de8-b5d7-4b06b43c6fde", "uri": "../sources/a29449fd-aa2f-4de8-b5d7-4b06b43c6fde.xml"}]}, "publicationAndOwnership": {"dataSetVersion": "00.03.100", "referenceToRegistrationAuthority": {"shortDescription": [{"value": "Institut Bauen und Umwelt e. V.", "lang": "en"}], "type": "contact data set", "refObjectId": "d111dbec-b024-4be5-86c5-752d6eb2cf95", "uri": "../contacts/d111dbec-b024-4be5-86c5-752d6eb2cf95.xml"}, "registrationNumber": "EPD-DOR-20210083-IBI1-EN", "referenceToOwnershipOfDataSet": {"shortDescription": [{"value": "dormakaba International Holding GmbH", "lang": "en"}], "type": "contact data set", "refObjectId": "33313944-7b37-498a-b458-25a295c1017d", "uri": "../contacts/33313944-7b37-498a-b458-25a295c1017d.xml"}, "copyright": true, "licenseType": "Free of charge for all users and uses", "accessRestrictions": [{"value": "None", "lang": "en"}], "other": {"anies": [{"name": "referenceToPublisher", "value": {"shortDescription": [{"value": "Institut Bauen und Umwelt e. V.", "lang": "en"}], "type": "contact data set", "refObjectId": "d111dbec-b024-4be5-86c5-752d6eb2cf95", "uri": "../contacts/d111dbec-b024-4be5-86c5-752d6eb2cf95.xml"}}]}}}, "exchanges": {"exchange": [{"dataSetInternalID": 0, "referenceToFlowDataSet": {"shortDescription": [{"value": "ST PRO Green RC (ST PRO Green RC)", "lang": "en"}], "type": "flow data set", "refObjectId": "75d7a4c5-a93c-18dd-91e6-15f8d47f649b", "uri": "../flows/75d7a4c5-a93c-18dd-91e6-15f8d47f649b.xml"}, "meanAmount": 1.0, "referencesToDataSource": {}, "referenceFlow": true, "resolvedFlowVersion": "00.03.000", "resultingflowAmount": 4.07, "flowProperties": [{"name": [{"lang": "de", "value": "Fläche"}, {"lang": "en", "value": "Area"}], "uuid": "93a60a56-a3c8-19da-a746-0800200c9a66", "referenceFlowProperty": true, "meanValue": 4.07, "referenceUnit": "qm", "unitGroupUUID": "c20a03d7-bd90-4569-bc94-66cfd364dfc8"}, {"name": [{"lang": "en", "value": "Weight"}], "uuid": "93a60a56-a3c8-11da-a746-0800200b9a66", "meanValue": 228.08}], "materialProperties": [{"name": "layer thickness", "value": "0.0245", "unit": "m", "unitDescription": "meters"}, {"name": "conversion factor to 1 kg", "value": "0.004", "unit": "-", "unitDescription": "Without unit"}, {"name": "grammage", "value": "56.03", "unit": "kg/m^2", "unitDescription": "kilograms per square meter"}], "typeOfFlow": "Product flow", "classification": {"classHierarchy": "Komponenten von Fenstern und Vorhangfassaden / Rahmen / Profile / Aluminium", "name": "OEKOBAU.DAT"}}, {"dataSetInternalID": 1, "referenceToFlowDataSet": {"shortDescription": [{"value": "Renewable primary energy as energy carrier (PERE)", "lang": "en"}, {"value": "Erneuerbare Primärenergie als Energieträger (PERE)", "lang": "de"}], "type": "flow data set", "refObjectId": "20f32be5-0398-4288-9b6d-accddd195317", "uri": "../flows/20f32be5-0398-4288-9b6d-accddd195317.xml"}, "exchange direction": "INPUT", "other": {"anies": [{"name": "referenceToUnitGroupDataSet", "value": {"shortDescription": [{"value": "MJ", "lang": "en"}], "type": "unit group data set", "refObjectId": "93a60a57-a3c8-11da-a746-0800200c9a66", "uri": "../unitgroups/93a60a57-a3c8-11da-a746-0800200c9a66.xml"}}, {"value": "2122.2976", "module": "A1-A3"}, {"value": "7.7", "module": "A4"}, {"value": "39.0624", "module": "A5"}, {"value": "3100", "module": "B6"}, {"value": "0.0653", "module": "C1"}, {"value": "0.551", "module": "C2"}, {"value": "4.56", "module": "C3"}, {"value": "0", "module": "C4"}, {"value": "-445", "module": "D"}]}, "resolvedFlowVersion": "38.00.000", "flowProperties": [], "typeOfFlow": "Other flow", "classification": {"classHierarchy": "Quantities", "name": "GaBiCategories"}}, {"dataSetInternalID": 2, "referenceToFlowDataSet": {"shortDescription": [{"value": "Renewable primary energy resources as material utilization (PERM)", "lang": "en"}, {"value": "Erneuerbare Primärenergie zur stofflichen Nutzung (PERM)", "lang": "de"}], "type": "flow data set", "refObjectId": "fb3ec0de-548d-4508-aea5-00b73bf6f702", "uri": "../flows/fb3ec0de-548d-4508-aea5-00b73bf6f702.xml"}, "exchange direction": "INPUT", "other": {"anies": [{"name": "referenceToUnitGroupDataSet", "value": {"shortDescription": [{"value": "MJ", "lang": "en"}], "type": "unit group data set", "refObjectId": "93a60a57-a3c8-11da-a746-0800200c9a66", "uri": "../unitgroups/93a60a57-a3c8-11da-a746-0800200c9a66.xml"}}, {"value": "37.7024", "module": "A1-A3"}, {"value": "0", "module": "A4"}, {"value": "-37.7024", "module": "A5"}, {"value": "0", "module": "B6"}, {"value": "0", "module": "C1"}, {"value": "0", "module": "C2"}, {"value": "0", "module": "C3"}, {"value": "0", "module": "C4"}, {"value": "0", "module": "D"}]}, "resolvedFlowVersion": "38.00.000", "flowProperties": [], "typeOfFlow": "Other flow", "classification": {"classHierarchy": "Quantities", "name": "GaBiCategories"}}, {"dataSetInternalID": 3, "referenceToFlowDataSet": {"shortDescription": [{"value": "Total use of renewable primary energy resources (PERT)", "lang": "en"}, {"value": "Total erneuerbare Primärenergie (PERT)", "lang": "de"}], "type": "flow data set", "refObjectId": "53f97275-fa8a-4cdd-9024-65936002acd0", "uri": "../flows/53f97275-fa8a-4cdd-9024-65936002acd0.xml"}, "exchange direction": "INPUT", "other": {"anies": [{"name": "referenceToUnitGroupDataSet", "value": {"shortDescription": [{"value": "MJ", "lang": "en"}], "type": "unit group data set", "refObjectId": "93a60a57-a3c8-11da-a746-0800200c9a66", "uri": "../unitgroups/93a60a57-a3c8-11da-a746-0800200c9a66.xml"}}, {"value": "2160", "module": "A1-A3"}, {"value": "7.7", "module": "A4"}, {"value": "1.36", "module": "A5"}, {"value": "3100", "module": "B6"}, {"value": "0.0653", "module": "C1"}, {"value": "0.551", "module": "C2"}, {"value": "4.56", "module": "C3"}, {"value": "0", "module": "C4"}, {"value": "-445", "module": "D"}]}, "resolvedFlowVersion": "38.00.000", "flowProperties": [], "typeOfFlow": "Other flow", "classification": {"classHierarchy": "Quantities / Environmental quantities / EPD EN 15804 / LCI indicators", "name": "GaBiCategories"}}, {"dataSetInternalID": 4, "referenceToFlowDataSet": {"shortDescription": [{"value": "Non renewable primary energy as energy carrier (PENRE)", "lang": "en"}, {"value": "Nicht-erneuerbare Primärenergie als Energieträger (PENRE)", "lang": "de"}], "type": "flow data set", "refObjectId": "ac857178-2b45-46ec-892a-a9a4332f0372", "uri": "../flows/ac857178-2b45-46ec-892a-a9a4332f0372.xml"}, "exchange direction": "INPUT", "other": {"anies": [{"name": "referenceToUnitGroupDataSet", "value": {"shortDescription": [{"value": "MJ", "lang": "en"}], "type": "unit group data set", "refObjectId": "93a60a57-a3c8-11da-a746-0800200c9a66", "uri": "../unitgroups/93a60a57-a3c8-11da-a746-0800200c9a66.xml"}}, {"value": "13019.3852529088", "module": "A1-A3"}, {"value": "137", "module": "A4"}, {"value": "10.844", "module": "A5"}, {"value": "7000", "module": "B6"}, {"value": "0.147", "module": "C1"}, {"value": "9.46", "module": "C2"}, {"value": "314.6703170912", "module": "C3"}, {"value": "0", "module": "C4"}, {"value": "-1670", "module": "D"}]}, "resolvedFlowVersion": "38.00.000", "flowProperties": [], "typeOfFlow": "Other flow", "classification": {"classHierarchy": "Quantities", "name": "GaBiCategories"}}, {"dataSetInternalID": 5, "referenceToFlowDataSet": {"shortDescription": [{"value": "Non renewable primary energy as material utilization (PENRM)", "lang": "en"}, {"value": "Nicht-erneuerbare Primärenergie zur stofflichen Nutzung (PENRM)", "lang": "de"}], "type": "flow data set", "refObjectId": "1421caa0-679d-4bf4-b282-0eb850ccae27", "uri": "../flows/1421caa0-679d-4bf4-b282-0eb850ccae27.xml"}, "exchange direction": "INPUT", "other": {"anies": [{"name": "referenceToUnitGroupDataSet", "value": {"shortDescription": [{"value": "MJ", "lang": "en"}], "type": "unit group data set", "refObjectId": "93a60a57-a3c8-11da-a746-0800200c9a66", "uri": "../unitgroups/93a60a57-a3c8-11da-a746-0800200c9a66.xml"}}, {"value": "280.6147470912", "module": "A1-A3"}, {"value": "0", "module": "A4"}, {"value": "-0.344", "module": "A5"}, {"value": "0", "module": "B6"}, {"value": "0", "module": "C1"}, {"value": "0", "module": "C2"}, {"value": "-280.2703170912", "module": "C3"}, {"value": "0", "module": "C4"}, {"value": "0", "module": "D"}]}, "resolvedFlowVersion": "38.00.000", "flowProperties": [], "typeOfFlow": "Other flow", "classification": {"classHierarchy": "Quantities", "name": "GaBiCategories"}}, {"dataSetInternalID": 6, "referenceToFlowDataSet": {"shortDescription": [{"value": "Total use of non renewable primary energy resources (PENRT)", "lang": "en"}, {"value": "Total nicht erneuerbare Primärenergie (PENRT)", "lang": "de"}], "type": "flow data set", "refObjectId": "06159210-646b-4c8d-8583-da9b3b95a6c1", "uri": "../flows/06159210-646b-4c8d-8583-da9b3b95a6c1.xml"}, "exchange direction": "INPUT", "other": {"anies": [{"name": "referenceToUnitGroupDataSet", "value": {"shortDescription": [{"value": "MJ", "lang": "en"}], "type": "unit group data set", "refObjectId": "93a60a57-a3c8-11da-a746-0800200c9a66", "uri": "../unitgroups/93a60a57-a3c8-11da-a746-0800200c9a66.xml"}}, {"value": "13300", "module": "A1-A3"}, {"value": "137", "module": "A4"}, {"value": "10.5", "module": "A5"}, {"value": "7000", "module": "B6"}, {"value": "0.147", "module": "C1"}, {"value": "9.46", "module": "C2"}, {"value": "34.4", "module": "C3"}, {"value": "0", "module": "C4"}, {"value": "-1670", "module": "D"}]}, "resolvedFlowVersion": "38.00.000", "flowProperties": [], "typeOfFlow": "Other flow", "classification": {"classHierarchy": "Quantities / Environmental quantities / EPD EN 15804 / LCI indicators", "name": "GaBiCategories"}}, {"dataSetInternalID": 7, "referenceToFlowDataSet": {"shortDescription": [{"value": "Use of secondary material (SM)", "lang": "en"}, {"value": "Einsatz von Sekundärstoffen (SM)", "lang": "de"}], "type": "flow data set", "refObjectId": "c6a1f35f-2d09-4f54-8dfb-97e502e1ce92", "uri": "../flows/c6a1f35f-2d09-4f54-8dfb-97e502e1ce92.xml"}, "exchange direction": "INPUT", "other": {"anies": [{"name": "referenceToUnitGroupDataSet", "value": {"shortDescription": [{"value": "kg", "lang": "en"}], "type": "unit group data set", "refObjectId": "ad38d542-3fe9-439d-9b95-2f5f7752acaf", "uri": "../unitgroups/ad38d542-3fe9-439d-9b95-2f5f7752acaf.xml"}}, {"value": "50.0768293888", "module": "A1-A3"}, {"value": "0", "module": "A4"}, {"value": "0", "module": "A5"}, {"value": "0", "module": "B6"}, {"value": "0", "module": "C1"}, {"value": "0", "module": "C2"}, {"value": "0", "module": "C3"}, {"value": "0", "module": "C4"}, {"value": "165.8386902504", "module": "D"}]}, "resolvedFlowVersion": "38.00.000", "flowProperties": [], "typeOfFlow": "Other flow", "classification": {"classHierarchy": "Quantities / Environmental quantities / EPD EN 15804 / LCI indicators", "name": "GaBiCategories"}}, {"dataSetInternalID": 8, "referenceToFlowDataSet": {"shortDescription": [{"value": "Use of renewable secondary fuels (RSF)", "lang": "en"}, {"value": "Erneuerbare Sekundärbrennstoffe (RSF)", "lang": "de"}], "type": "flow data set", "refObjectId": "64333088-a55f-4aa2-9a31-c10b07816787", "uri": "../flows/64333088-a55f-4aa2-9a31-c10b07816787.xml"}, "exchange direction": "INPUT", "other": {"anies": [{"name": "referenceToUnitGroupDataSet", "value": {"shortDescription": [{"value": "MJ", "lang": "en"}], "type": "unit group data set", "refObjectId": "93a60a57-a3c8-11da-a746-0800200c9a66", "uri": "../unitgroups/93a60a57-a3c8-11da-a746-0800200c9a66.xml"}}, {"value": "0", "module": "A1-A3"}, {"value": "0", "module": "A4"}, {"value": "0", "module": "A5"}, {"value": "0", "module": "B6"}, {"value": "0", "module": "C1"}, {"value": "0", "module": "C2"}, {"value": "0", "module": "C3"}, {"value": "0", "module": "C4"}, {"value": "0", "module": "D"}]}, "resolvedFlowVersion": "38.00.000", "flowProperties": [], "typeOfFlow": "Other flow", "classification": {"classHierarchy": "Quantities / Environmental quantities / EPD EN 15804 / LCI indicators", "name": "GaBiCategories"}}, {"dataSetInternalID": 9, "referenceToFlowDataSet": {"shortDescription": [{"value": "Use of non renewable secondary fuels (NRSF)", "lang": "en"}, {"value": "Nicht erneuerbare Sekundärbrennstoffe (NRSF)", "lang": "de"}], "type": "flow data set", "refObjectId": "89def144-d39a-4287-b86f-efde453ddcb2", "uri": "../flows/89def144-d39a-4287-b86f-efde453ddcb2.xml"}, "exchange direction": "INPUT", "other": {"anies": [{"name": "referenceToUnitGroupDataSet", "value": {"shortDescription": [{"value": "MJ", "lang": "en"}], "type": "unit group data set", "refObjectId": "93a60a57-a3c8-11da-a746-0800200c9a66", "uri": "../unitgroups/93a60a57-a3c8-11da-a746-0800200c9a66.xml"}}, {"value": "0", "module": "A1-A3"}, {"value": "0", "module": "A4"}, {"value": "0", "module": "A5"}, {"value": "0", "module": "B6"}, {"value": "0", "module": "C1"}, {"value": "0", "module": "C2"}, {"value": "0", "module": "C3"}, {"value": "0", "module": "C4"}, {"value": "0", "module": "D"}]}, "resolvedFlowVersion": "38.00.000", "flowProperties": [], "typeOfFlow": "Other flow", "classification": {"classHierarchy": "Quantities / Environmental quantities / EPD EN 15804 / LCI indicators", "name": "GaBiCategories"}}, {"dataSetInternalID": 10, "referenceToFlowDataSet": {"shortDescription": [{"value": "Use of net fresh water (FW)", "lang": "en"}, {"value": "Einsatz von Süßwasserressourcen (FW)", "lang": "de"}], "type": "flow data set", "refObjectId": "3cf952c8-f3a4-461d-8c96-96456ca62246", "uri": "../flows/3cf952c8-f3a4-461d-8c96-96456ca62246.xml"}, "exchange direction": "INPUT", "other": {"anies": [{"name": "referenceToUnitGroupDataSet", "value": {"shortDescription": [{"value": "m^3", "lang": "en"}], "type": "unit group data set", "refObjectId": "cd950537-0a98-4044-9ba7-9f9a68d0a504", "uri": "../unitgroups/cd950537-0a98-4044-9ba7-9f9a68d0a504.xml"}}, {"value": "10.1", "module": "A1-A3"}, {"value": "0.00892", "module": "A4"}, {"value": "0.0141", "module": "A5"}, {"value": "3.59", "module": "B6"}, {"value": "7.56E-05", "module": "C1"}, {"value": "0.000595", "module": "C2"}, {"value": "0.093", "module": "C3"}, {"value": "0", "module": "C4"}, {"value": "-4.32", "module": "D"}]}, "resolvedFlowVersion": "38.00.000", "flowProperties": [], "typeOfFlow": "Other flow", "classification": {"classHierarchy": "Quantities / Environmental quantities / EPD EN 15804 / LCI indicators", "name": "GaBiCategories"}}, {"dataSetInternalID": 11, "referenceToFlowDataSet": {"shortDescription": [{"value": "Hazardous waste disposed (HWD)", "lang": "en"}, {"value": "Gefährlicher Abfall zur Deponie (HWD)", "lang": "de"}], "type": "flow data set", "refObjectId": "430f9e0f-59b2-46a0-8e0d-55e0e84948fc", "uri": "../flows/430f9e0f-59b2-46a0-8e0d-55e0e84948fc.xml"}, "exchange direction": "OUTPUT", "other": {"anies": [{"name": "referenceToUnitGroupDataSet", "value": {"shortDescription": [{"value": "kg", "lang": "en"}], "type": "unit group data set", "refObjectId": "ad38d542-3fe9-439d-9b95-2f5f7752acaf", "uri": "../unitgroups/ad38d542-3fe9-439d-9b95-2f5f7752acaf.xml"}}, {"value": "0.115", "module": "A1-A3"}, {"value": "6.38E-06", "module": "A4"}, {"value": "2.41E-08", "module": "A5"}, {"value": "2.9E-06", "module": "B6"}, {"value": "6.1E-11", "module": "C1"}, {"value": "4.12E-07", "module": "C2"}, {"value": "5.24E-08", "module": "C3"}, {"value": "0", "module": "C4"}, {"value": "-2.78E-06", "module": "D"}]}, "resolvedFlowVersion": "38.00.000", "flowProperties": [], "typeOfFlow": "Other flow", "classification": {"classHierarchy": "Quantities / Environmental quantities / EPD EN 15804 / LCI indicators", "name": "GaBiCategories"}}, {"dataSetInternalID": 12, "referenceToFlowDataSet": {"shortDescription": [{"value": "Non hazardous waste disposed (NHWD)", "lang": "en"}, {"value": "Entsorgter nicht gefährlicher Abfall (NHWD)", "lang": "de"}], "type": "flow data set", "refObjectId": "b29ef66b-e286-4afa-949f-62f1a7b4d7fa", "uri": "../flows/b29ef66b-e286-4afa-949f-62f1a7b4d7fa.xml"}, "exchange direction": "OUTPUT", "other": {"anies": [{"name": "referenceToUnitGroupDataSet", "value": {"shortDescription": [{"value": "kg", "lang": "en"}], "type": "unit group data set", "refObjectId": "ad38d542-3fe9-439d-9b95-2f5f7752acaf", "uri": "../unitgroups/ad38d542-3fe9-439d-9b95-2f5f7752acaf.xml"}}, {"value": "281", "module": "A1-A3"}, {"value": "0.021", "module": "A4"}, {"value": "0.139", "module": "A5"}, {"value": "4.96", "module": "B6"}, {"value": "0.000105", "module": "C1"}, {"value": "0.00156", "module": "C2"}, {"value": "3.21", "module": "C3"}, {"value": "0", "module": "C4"}, {"value": "-20", "module": "D"}]}, "resolvedFlowVersion": "38.00.000", "flowProperties": [], "typeOfFlow": "Other flow", "classification": {"classHierarchy": "Quantities / Environmental quantities / EPD EN 15804 / LCI indicators", "name": "GaBiCategories"}}, {"dataSetInternalID": 13, "referenceToFlowDataSet": {"shortDescription": [{"value": "Radioactive waste disposed (RWD)", "lang": "en"}, {"value": "Entsorgter radioaktiver Abfall (RWD)", "lang": "de"}], "type": "flow data set", "refObjectId": "3449546e-52ad-4b39-b809-9fb77cea8ff6", "uri": "../flows/3449546e-52ad-4b39-b809-9fb77cea8ff6.xml"}, "exchange direction": "OUTPUT", "other": {"anies": [{"name": "referenceToUnitGroupDataSet", "value": {"shortDescription": [{"value": "kg", "lang": "en"}], "type": "unit group data set", "refObjectId": "ad38d542-3fe9-439d-9b95-2f5f7752acaf", "uri": "../unitgroups/ad38d542-3fe9-439d-9b95-2f5f7752acaf.xml"}}, {"value": "0.679", "module": "A1-A3"}, {"value": "0.00017", "module": "A4"}, {"value": "0.000315", "module": "A5"}, {"value": "1.06", "module": "B6"}, {"value": "2.24E-05", "module": "C1"}, {"value": "1.6E-05", "module": "C2"}, {"value": "0.000549", "module": "C3"}, {"value": "0", "module": "C4"}, {"value": "-0.0771", "module": "D"}]}, "resolvedFlowVersion": "38.00.000", "flowProperties": [], "typeOfFlow": "Other flow", "classification": {"classHierarchy": "Quantities / Environmental quantities / EPD EN 15804 / LCI indicators", "name": "GaBiCategories"}}, {"dataSetInternalID": 14, "referenceToFlowDataSet": {"shortDescription": [{"value": "Components for re-use (CRU)", "lang": "en"}, {"value": "Komponenten für die Wiederverwendung (CRU)", "lang": "de"}], "type": "flow data set", "refObjectId": "a2b32f97-3fc7-4af2-b209-525bc6426f33", "uri": "../flows/a2b32f97-3fc7-4af2-b209-525bc6426f33.xml"}, "exchange direction": "OUTPUT", "other": {"anies": [{"name": "referenceToUnitGroupDataSet", "value": {"shortDescription": [{"value": "kg", "lang": "en"}], "type": "unit group data set", "refObjectId": "ad38d542-3fe9-439d-9b95-2f5f7752acaf", "uri": "../unitgroups/ad38d542-3fe9-439d-9b95-2f5f7752acaf.xml"}}, {"value": "0", "module": "A1-A3"}, {"value": "0", "module": "A4"}, {"value": "0", "module": "A5"}, {"value": "0", "module": "B6"}, {"value": "0", "module": "C1"}, {"value": "0", "module": "C2"}, {"value": "0", "module": "C3"}, {"value": "0", "module": "C4"}, {"value": "0", "module": "D"}]}, "resolvedFlowVersion": "38.00.000", "flowProperties": [], "typeOfFlow": "Other flow", "classification": {"classHierarchy": "Quantities / Environmental quantities / EPD EN 15804 / LCI indicators", "name": "GaBiCategories"}}, {"dataSetInternalID": 15, "referenceToFlowDataSet": {"shortDescription": [{"value": "Materials for recycling (MFR)", "lang": "en"}, {"value": "Stoffe zum Recycling (MFR)", "lang": "de"}], "type": "flow data set", "refObjectId": "d7fe48a5-4103-49c8-9aae-b0b5dfdbd6ae", "uri": "../flows/d7fe48a5-4103-49c8-9aae-b0b5dfdbd6ae.xml"}, "exchange direction": "OUTPUT", "other": {"anies": [{"name": "referenceToUnitGroupDataSet", "value": {"shortDescription": [{"value": "kg", "lang": "en"}], "type": "unit group data set", "refObjectId": "ad38d542-3fe9-439d-9b95-2f5f7752acaf", "uri": "../unitgroups/ad38d542-3fe9-439d-9b95-2f5f7752acaf.xml"}}, {"value": "9.6360218016", "module": "A1-A3"}, {"value": "0", "module": "A4"}, {"value": "0", "module": "A5"}, {"value": "0", "module": "B6"}, {"value": "0", "module": "C1"}, {"value": "0", "module": "C2"}, {"value": "213.0528172184", "module": "C3"}, {"value": "0", "module": "C4"}, {"value": "0", "module": "D"}]}, "resolvedFlowVersion": "38.00.000", "flowProperties": [], "typeOfFlow": "Other flow", "classification": {"classHierarchy": "Quantities / Environmental quantities / EPD EN 15804 / LCI indicators", "name": "GaBiCategories"}}, {"dataSetInternalID": 16, "referenceToFlowDataSet": {"shortDescription": [{"value": "Materials for energy recovery (MER)", "lang": "en"}, {"value": "Stoffe für die Energierückgewinnung (MER)", "lang": "de"}], "type": "flow data set", "refObjectId": "59a9181c-3aaf-46ee-8b13-2b3723b6e447", "uri": "../flows/59a9181c-3aaf-46ee-8b13-2b3723b6e447.xml"}, "exchange direction": "OUTPUT", "other": {"anies": [{"name": "referenceToUnitGroupDataSet", "value": {"shortDescription": [{"value": "kg", "lang": "en"}], "type": "unit group data set", "refObjectId": "ad38d542-3fe9-439d-9b95-2f5f7752acaf", "uri": "../unitgroups/ad38d542-3fe9-439d-9b95-2f5f7752acaf.xml"}}, {"value": "3.0085392216", "module": "A1-A3"}, {"value": "0", "module": "A4"}, {"value": "2.9808", "module": "A5"}, {"value": "0", "module": "B6"}, {"value": "0", "module": "C1"}, {"value": "0", "module": "C2"}, {"value": "14.8311327584", "module": "C3"}, {"value": "0", "module": "C4"}, {"value": "0", "module": "D"}]}, "resolvedFlowVersion": "38.00.000", "flowProperties": [], "typeOfFlow": "Other flow", "classification": {"classHierarchy": "Quantities / Environmental quantities / EPD EN 15804 / LCI indicators", "name": "GaBiCategories"}}, {"dataSetInternalID": 17, "referenceToFlowDataSet": {"shortDescription": [{"value": "Exported electrical energy (EEE)", "lang": "en"}, {"value": "Exportierte elektrische Energie (EEE)", "lang": "de"}], "type": "flow data set", "refObjectId": "4da0c987-2b76-40d6-9e9e-82a017aaaf29", "uri": "../flows/4da0c987-2b76-40d6-9e9e-82a017aaaf29.xml"}, "exchange direction": "OUTPUT", "other": {"anies": [{"name": "referenceToUnitGroupDataSet", "value": {"shortDescription": [{"value": "MJ", "lang": "en"}], "type": "unit group data set", "refObjectId": "93a60a57-a3c8-11da-a746-0800200c9a66", "uri": "../unitgroups/93a60a57-a3c8-11da-a746-0800200c9a66.xml"}}, {"value": "0", "module": "A1-A3"}, {"value": "0", "module": "A4"}, {"value": "6.57226", "module": "A5"}, {"value": "0", "module": "B6"}, {"value": "0", "module": "C1"}, {"value": "0", "module": "C2"}, {"value": "52.838", "module": "C3"}, {"value": "0", "module": "C4"}, {"value": "0", "module": "D"}]}, "resolvedFlowVersion": "38.00.000", "flowProperties": [], "typeOfFlow": "Other flow", "classification": {"classHierarchy": "Quantities / Environmental quantities / EPD EN 15804 / LCI indicators", "name": "GaBiCategories"}}, {"dataSetInternalID": 18, "referenceToFlowDataSet": {"shortDescription": [{"value": "Exported thermal energy (EET)", "lang": "en"}, {"value": "Exportierte thermische Energie (EET)", "lang": "de"}], "type": "flow data set", "refObjectId": "98daf38a-7a79-46d3-9a37-2b7bd0955810", "uri": "../flows/98daf38a-7a79-46d3-9a37-2b7bd0955810.xml"}, "exchange direction": "OUTPUT", "other": {"anies": [{"name": "referenceToUnitGroupDataSet", "value": {"shortDescription": [{"value": "MJ", "lang": "en"}], "type": "unit group data set", "refObjectId": "93a60a57-a3c8-11da-a746-0800200c9a66", "uri": "../unitgroups/93a60a57-a3c8-11da-a746-0800200c9a66.xml"}}, {"value": "0", "module": "A1-A3"}, {"value": "0", "module": "A4"}, {"value": "11.91265", "module": "A5"}, {"value": "0", "module": "B6"}, {"value": "0", "module": "C1"}, {"value": "0", "module": "C2"}, {"value": "110.7", "module": "C3"}, {"value": "0", "module": "C4"}, {"value": "0", "module": "D"}]}, "resolvedFlowVersion": "38.00.000", "flowProperties": [], "typeOfFlow": "Other flow", "classification": {"classHierarchy": "Quantities / Environmental quantities / EPD EN 15804 / LCI indicators", "name": "GaBiCategories"}}]}, "LCIAResults": {"LCIAResult": [{"referenceToLCIAMethodDataSet": {"shortDescription": [{"value": "Global warming potential (GWP)", "lang": "en"}, {"value": "Globales Erwärmungspotenzial (GWP)", "lang": "de"}], "type": "LCIA method data set", "refObjectId": "77e416eb-a363-4258-a04e-171d843a6460", "uri": "../lciamethods/77e416eb-a363-4258-a04e-171d843a6460.xml"}, "other": {"anies": [{"name": "referenceToUnitGroupDataSet", "value": {"shortDescription": [{"value": "kg CO_(2) eq", "lang": "en"}], "type": "unit group data set", "refObjectId": "1ebf3012-d0db-4de2-aefd-ef30cedb0be1", "uri": "../unitgroups/1ebf3012-d0db-4de2-aefd-ef30cedb0be1.xml"}}, {"value": "844", "module": "A1-A3"}, {"value": "10", "module": "A4"}, {"value": "4.99", "module": "A5"}, {"value": "390", "module": "B6"}, {"value": "0.00822", "module": "C1"}, {"value": "0.69", "module": "C2"}, {"value": "31.5", "module": "C3"}, {"value": "0", "module": "C4"}, {"value": "-130", "module": "D"}]}}, {"referenceToLCIAMethodDataSet": {"shortDescription": [{"value": "Depletion potential of the stratospheric ozone layer (ODP)", "lang": "en"}, {"value": "Abbau Potential der stratosphärischen Ozonschicht (ODP)", "lang": "de"}], "type": "LCIA method data set", "refObjectId": "06dcd26f-025f-401a-a7c1-5e457eb54637", "uri": "../lciamethods/06dcd26f-025f-401a-a7c1-5e457eb54637.xml"}, "other": {"anies": [{"name": "referenceToUnitGroupDataSet", "value": {"shortDescription": [{"value": "kg CFC11 eq", "lang": "en"}], "type": "unit group data set", "refObjectId": "88054749-b0a6-47ea-a82b-dc5b29326512", "uri": "../unitgroups/88054749-b0a6-47ea-a82b-dc5b29326512.xml"}}, {"value": "1.23E-05", "module": "A1-A3"}, {"value": "1.65E-15", "module": "A4"}, {"value": "5.95E-15", "module": "A5"}, {"value": "1.17E-11", "module": "B6"}, {"value": "2.46E-16", "module": "C1"}, {"value": "2.17E-16", "module": "C2"}, {"value": "1.64E-07", "module": "C3"}, {"value": "0", "module": "C4"}, {"value": "-4.84E-08", "module": "D"}]}}, {"referenceToLCIAMethodDataSet": {"shortDescription": [{"value": "Acidification potential of land and water (AP)", "lang": "en"}, {"value": "Versauerungspotenzial von Boden und Wasser (AP)", "lang": "de"}], "type": "LCIA method data set", "refObjectId": "b4274add-93b7-4905-a5e4-2e878c4e4216", "uri": "../lciamethods/b4274add-93b7-4905-a5e4-2e878c4e4216.xml"}, "other": {"anies": [{"name": "referenceToUnitGroupDataSet", "value": {"shortDescription": [{"value": "kg SO_(2) eq", "lang": "en"}], "type": "unit group data set", "refObjectId": "bc50c624-a9bc-45b1-a9b0-e6b10d00476f", "uri": "../unitgroups/bc50c624-a9bc-45b1-a9b0-e6b10d00476f.xml"}}, {"value": "5.28", "module": "A1-A3"}, {"value": "0.0423", "module": "A4"}, {"value": "0.00223", "module": "A5"}, {"value": "0.819", "module": "B6"}, {"value": "1.73E-05", "module": "C1"}, {"value": "0.00294", "module": "C2"}, {"value": "0.0196", "module": "C3"}, {"value": "0", "module": "C4"}, {"value": "-0.537", "module": "D"}]}}, {"referenceToLCIAMethodDataSet": {"shortDescription": [{"value": "Eutrophication potential (EP)", "lang": "en"}, {"value": "Eutrophierungspotenzial (EP)", "lang": "de"}], "type": "LCIA method data set", "refObjectId": "f58827d0-b407-4ec6-be75-8b69efb98a0f", "uri": "../lciamethods/f58827d0-b407-4ec6-be75-8b69efb98a0f.xml"}, "other": {"anies": [{"name": "referenceToUnitGroupDataSet", "value": {"shortDescription": [{"value": "kg PO_(4)^(3) eq", "lang": "en"}], "type": "unit group data set", "refObjectId": "67b5401d-873c-485f-bcf3-6ae83b918822", "uri": "../unitgroups/67b5401d-873c-485f-bcf3-6ae83b918822.xml"}}, {"value": "0.982", "module": "A1-A3"}, {"value": "0.0106", "module": "A4"}, {"value": "0.000336", "module": "A5"}, {"value": "0.0906", "module": "B6"}, {"value": "1.91E-06", "module": "C1"}, {"value": "0.000734", "module": "C2"}, {"value": "0.0179", "module": "C3"}, {"value": "0", "module": "C4"}, {"value": "-0.0569", "module": "D"}]}}, {"referenceToLCIAMethodDataSet": {"shortDescription": [{"value": "Formation potential of tropospheric ozone photochemical oxidants (POCP)", "lang": "en"}, {"value": "Bildungspotential für troposphärisches Ozon (POCP)", "lang": "de"}], "type": "LCIA method data set", "refObjectId": "1e84a202-dae6-42aa-9e9d-71ea48b8be00", "uri": "../lciamethods/1e84a202-dae6-42aa-9e9d-71ea48b8be00.xml"}, "other": {"anies": [{"name": "referenceToUnitGroupDataSet", "value": {"shortDescription": [{"value": "kg Ethen eq", "lang": "en"}], "type": "unit group data set", "refObjectId": "01c26c17-9a76-406e-8295-f17b55fd909e", "uri": "../unitgroups/01c26c17-9a76-406e-8295-f17b55fd909e.xml"}}, {"value": "0.324", "module": "A1-A3"}, {"value": "-0.0178", "module": "A4"}, {"value": "0.000201", "module": "A5"}, {"value": "0.0583", "module": "B6"}, {"value": "1.23E-06", "module": "C1"}, {"value": "-0.0011", "module": "C2"}, {"value": "0.00156", "module": "C3"}, {"value": "0", "module": "C4"}, {"value": "-0.0408", "module": "D"}]}}, {"referenceToLCIAMethodDataSet": {"shortDescription": [{"value": "Abiotic depletion potential for non fossil resources (ADPE)", "lang": "en"}, {"value": "Potenzial für den abiotischen Abbau nicht fossiler Ressourcen (ADPE)", "lang": "de"}], "type": "LCIA method data set", "refObjectId": "f7c73bb9-ab1a-4249-9c6d-379a0de6f67e", "uri": "../lciamethods/f7c73bb9-ab1a-4249-9c6d-379a0de6f67e.xml"}, "other": {"anies": [{"name": "referenceToUnitGroupDataSet", "value": {"shortDescription": [{"value": "kg Sb eq", "lang": "en"}], "type": "unit group data set", "refObjectId": "54ccd2d9-a32a-4fc2-923d-f2c8c93e89d4", "uri": "../unitgroups/54ccd2d9-a32a-4fc2-923d-f2c8c93e89d4.xml"}}, {"value": "0.0649", "module": "A1-A3"}, {"value": "8.34E-07", "module": "A4"}, {"value": "2.35E-05", "module": "A5"}, {"value": "0.00013", "module": "B6"}, {"value": "2.75E-09", "module": "C1"}, {"value": "6.49E-08", "module": "C2"}, {"value": "6.3E-05", "module": "C3"}, {"value": "0", "module": "C4"}, {"value": "-0.00629", "module": "D"}]}}, {"referenceToLCIAMethodDataSet": {"shortDescription": [{"value": "Abiotic depletion potential for fossil resources (ADPF)", "lang": "en"}, {"value": "Potenzial für den abiotischen Abbau fossiler Brennstoffe (ADPF)", "lang": "de"}], "type": "LCIA method data set", "refObjectId": "804ebcdf-309d-4098-8ed8-fdaf2f389981", "uri": "../lciamethods/804ebcdf-309d-4098-8ed8-fdaf2f389981.xml"}, "other": {"anies": [{"name": "referenceToUnitGroupDataSet", "value": {"shortDescription": [{"value": "MJ", "lang": "en"}], "type": "unit group data set", "refObjectId": "93a60a57-a3c8-11da-a746-0800200c9a66", "uri": "../unitgroups/93a60a57-a3c8-11da-a746-0800200c9a66.xml"}}, {"value": "11200", "module": "A1-A3"}, {"value": "137", "module": "A4"}, {"value": "9.73", "module": "A5"}, {"value": "4320", "module": "B6"}, {"value": "0.0911", "module": "C1"}, {"value": "9.42", "module": "C2"}, {"value": "30.4", "module": "C3"}, {"value": "0", "module": "C4"}, {"value": "-1480", "module": "D"}]}}]}, "otherAttributes": {"{http://www.indata.network/EPD/2019}epd-version": "1.2"}, "version": "1.1", "locations": "../ILCDLocations.xml"}