{"processInformation": {"dataSetInformation": {"UUID": "ed6d477a-a4c3-4a96-9a28-24e256db88e3", "name": {"baseName": [{"value": "Stainless Steel screws", "lang": "en"}, {"value": "Schrauben aus Edelstahl", "lang": "de"}], "functionalUnitFlowProperties": [{"lang": "en"}]}, "classificationInformation": {"classification": [{"class": [{"value": "Metalle", "level": 0, "classId": "4"}, {"value": "Edelstahl", "level": 1, "classId": "4.2"}, {"value": "Befestigungsmittel", "level": 2, "classId": "4.2.04"}], "name": "OEKOBAU.DAT"}, {"class": [{"value": "02 Building products", "level": 0}, {"value": "Fixings", "level": 1}, {"value": "Screws", "level": 2}], "name": "IBUCategories"}]}, "generalComment": [{"value": "Dowel-type fasteners with thread, e.g. screws made of stainless steel, are fasteners that can predominantly be used for fastening two or more components. The materials to be fastened or screw-in surfaces can be made of wood, wood materials, plastic, aluminium, steel, stainless steel or other metals.\n\nPin-shaped connectors, such as screws, are generally manufactured from a wire (stainless steel) and provided with a head on one component side to be tightened. Depending on the application, it can have different shapes, e.g. countersunk head, round head, hexagon head or washer head. For anchoring the pin-shaped connectors, a thread is formed on the opposite side. The thread shape (e.g. wood thread or metric thread) is matched to the screw-in surface and can be designed differently in terms of thread height, thread angle or thread pitch. The point design of the dowel-type fasteners with thread is matched to the application, e.g. wooden tip, drill tip or blunt shape. For protection against corrosion or e.g. for setting a sliding friction, the pin-shaped connectors can be provided with different coatings, for example, anti-skid coating. \n\nDepending on the application, the additional use of suitable steel or stainless steel seals as well as EPDM seals (ethylene-propylene-diene rubber), washers or nuts is provided. Depending on the application, the dowel-type fasteners with thread can be subject to legal national or European requirements such as the Construction Products Regulation. For example, the following documentation possibilities may be available:", "lang": "en"}, {"value": "Bei stiftförmigen Verbindungsmitteln mit Gewinde z.B. Schrauben aus Edelstahl, handelt es sich um Verbindungsmittel, die überwiegend zur Befestigung zweier oder mehrerer Bauteile verwendet werden können. Die zu befestigenden Materialien oder Einschraubuntergründe können aus den Materialien Holz, Holzwerkstoffe, Kunststoff, Aluminium, Stahl, Edelstahl oder anderen Metallen sein.", "lang": "de"}]}, "quantitativeReference": {"referenceToReferenceFlow": [0]}, "time": {"referenceYear": 2024, "dataSetValidUntil": 2029, "other": {"anies": [{"name": "publicationDateOfEPD", "value": 1710979200000}]}}, "geography": {"locationOfOperationSupplyOrProduction": {"location": "RER"}}, "technology": {"technologyDescriptionAndIncludedProcesses": [{"value": "Pin-shaped connectors, such as screws, are generally manufactured from a wire (stainless steel) and provided with a head on one component side to be tightened. Depending on the application, it can have different shapes, e.g. countersunk head, round head, hexagon head or washer head. For anchoring the pin-shaped connectors, a thread is formed on the opposite side. The thread shape (e.g. wood thread or metric thread) is matched to the screw-in surface and can be designed differently in terms of thread height, thread angle or thread pitch. The point design of the dowel-type fasteners with thread is matched to the application, e.g. wooden tip, drill tip or blunt shape. For protection against corrosion or e.g. for setting a sliding friction, the pin-shaped connectors can be provided with different coatings, for example anti-skid coating. Currently, mainly the following production methods are used to produce dowel-type fasteners with thread: cold or hot extrusion processes with multi-stage pressing tools. The starting material is delivered as coiled wire on spools and is uncoiled and straightened in the upstream plant. Modern cold and hot extrusion presses operate in multiple stages, i.e. several steps are carried out in a single operation, such as shearing of the blank, preforming of the screw head, final upsetting, deburring and reduction of the threaded part. In a next step, the thread of the screw is formed without cutting using a thread rolling machine. For self-drilling screws, pinching of the drill tip takes place before thread rolling. Between each working step, the parts are washed in a washing facility specially provided for this purpose. Finally, the screw surface is coated. \nTechnical data: \nStructural data for the respective dowel-type fasteners with thread are provided in the corresponding approvals and technical drawings, as shown below in an excerpt from ETA 11/0190 (ASSY) for wood screws. \nDeclared unit: \n1 kg average screws made of stainless steel:", "lang": "en"}, {"value": "Stiftförmige Verbindungsmittel wie beispielsweise Schrauben werden in der Regel aus einem Draht (Edelstahl) gefertigt und an der anzuziehenden Bauteilseite mit einem Kopf versehen. Dieser kann je nach Anwendung unterschiedlich ausgeformt sein z.B. Senkkopf, Linsenkopf, Sechskantkopf oder Scheibenkopf. Zur Verankerung des stiftförmigen Verbindungsmittels erfolgt auf der gegenüberliegenden Seite die Ausformung eines Gewindes. Die Gewindeausformung (z.B. Holzgewinde oder metrisches Gewinde) ist auf den Einschraubuntergrund abgestimmt und kann unterschiedlich hinsichtlich Gewindehöhe, Flankenwinkel oder Gewindesteigung ausgeformt sein. Die Spitzenausformung des stiftförmigen Verbindungsmittels ist auf die Anwendung abgestimmt z.B. Holzspitze, Bohrspitze oder stumpfe Ausformung. Zum Schutz vor Korrosion oder z.B. zur Einstellung einer Gleitreibung können die stiftförmigen Verbindungsmittel mit unterschiedlichen Überzügen z.B. Gleitschutzmittel versehen sein.\n\nZur Herstellung von stiftförmige Verbindungsmittel mit Gewinde werden derzeit hauptsächlich folgende Produktionsverfahren eingesetzt: Kalt- oder Warmfließpressverfahren mit mehrstufigen Presswerkszeugen. Das Ausgangsmaterial wird als aufgewickelter Draht auf Spulen angeliefert und in der vorgeschalteten Anlage abgewickelt und gerichtet. Moderne Kalt- und Warmfließpressen arbeiten mehrstufig. d.h. mehrere Arbeitsschritte in einem Arbeitsgang werden dabei durchgeführt, wie z. B. Abscheren des Rohlings, Vorformen des Schraubenkopfes, Fertigstauchen, Entgraten und reduzieren des Gewindeteils. Im nächsten Schritt wird das Gewinde der Schraube mit einer Gewindewalzmaschine spanlos verformt. Bei selbstbohrenden Schrauben erfolgt vor dem Gewindewalzen das Kneifen der Bohrspitze. Zwischen jedem Arbeitsschritt werden die Teile in einer speziell dafür vorgesehenen Waschanlage gewaschen. Abschließend wird die Schraubenoberfläche beschichtet. \nTechnische Daten: \nBautechnische Daten zu den jeweiligen stiftförmigen Verbindungsmittel mit Gewinde sind in den entsprechenden Zulassungen sowie technischen Zeichnungen hinterlegt, nachfolgend beispielhaft dargestellt an einem Auszug aus der ETA 11/0190 (ASSY) für Holzschrauben. \nDeklarierte Einheit: \n1 kg durchschnittliche Schrauben aus Edelstahl", "lang": "de"}], "technologicalApplicability": [{"value": "Timber screws, chipboard screws, drilling and tapping screws, plastic screws and dowel-type fasteners with thread made of stainless steel are used when fastening two or more components. Depending on the type of screw, these products are generally used for fastening components made of wood, steel or plastic. Possible application examples include timber construction, steel construction, indoor/outdoor use, furniture applications or window construction. Examples of Wrth product groups are ASSY, Pias and Piasta screws.", "lang": "en"}, {"value": "Holzbauschrauben, Spanplattenschrauben, Bohr- und Blechschrauben, Schrauben für Kunststoffe und stiftförmige Verbindungsmittel mit Gewinde aus Edelstahl kommen dann zum Einsatz, wenn eine Befestigung zweier oder mehrerer Bauteile vorgesehen ist. Je nach Schraubentyp werden diese Produkte in der Regel zur Befestigung der Bauteile aus Holz, Stahl oder Kunststoff verwendet. Mögliche Anwendungsbeispiele können der Holzbau, Stahlbau, die Verwendung im Innen-/ oder Außenbereich, für Möbelanwendungen oder den Fensterbau sein. ", "lang": "de"}]}}, "modellingAndValidation": {"LCIMethodAndAllocation": {"typeOfDataSet": "EPD", "referenceToLCAMethodDetails": [{"shortDescription": [{"value": "Screws.pdf", "lang": "en"}], "type": "source data set", "refObjectId": "8f1b97d0-a8a4-411d-bba3-7af0d2350cac"}], "other": {"anies": [{"name": "subType", "value": "specific dataset"}]}}, "dataSourcesTreatmentAndRepresentativeness": {"referenceToDataSource": [{"shortDescription": [{"value": "GaBi Database (all versions)", "lang": "en"}], "type": "source data set", "refObjectId": "28d74cc0-db8b-4d7e-bc44-5f6d56ce0c4a"}, {"shortDescription": [{"value": "Sphera MLC (fka GaBi) CUP 2023.01", "lang": "en"}], "type": "source data set", "refObjectId": "6bcd5bfa-3623-48ab-a52b-6d5be8db82ed"}], "useAdviceForDataSet": [{"value": "Scope: \nThis EPD relates to timber screws, chipboard screws, drilling and tapping screws, screws for plastics, metric screws and dowel-type fasteners with thread made of steel or stainless steel. Depending on the type of screw, these products are generally used for fastening two or more components made of wood, steel or plastic.\n\nThe declared environmental data related to 1 kg of stainless steel are based on a weighted average stainless steel screws in a Wrth manufacturing plant, SWG Schraubenwerk Gaisbach GmbH and internationalized with generic data. The holder of the declaration shall be liable for the underlying information and supporting documents; any liability of IBU (Institut Bauen und Umwelt e. V.) with regard to manufacturer information, life cycle assessment data and supporting documents is hereby excluded. The EPD (Environmental Product Declaration) was created in accordance with EN 15804 + A2: 2022-03. In the following, the standard is referred to in simplified form as EN 15804. \nSystem boundary: \nType of the EPD: cradle-to-gate - with options, modules C1-C4 and module D (A1-A3 + C + D and additional modules: A4, A5).\n\nProduction Stage (A1-A3): The Product stage includes:\n· A1 Raw material supply and processing (mainly steel),\n· A2 Transport of raw materials to the manufacturer,\n· A3 Production of Stainless steel screws (incl. energy provision, treatment of production waste, production of packaging materials).\n\nConstruction stage (A4-A5): The construction process stage includes:\n· A4 transport to the construction site 100 km by truck,\n· A5 Disposal of the packaging and installation of the Stainless steel screw.\n\nEnd-of-life stage (C1-C4): The end-of-life stage includes:\n· C1 machine-assisted de- construction (Hand-screwdriver; battery operated)\n· C2 transport to waste processing; 50 km with truck Transport distance can be adjusted at building level if necessary (e.g., for 100 km actual transport distance: multiply LCA values by factor 2)\n· C3 waste processing for recycling of Stainless steel.\n· C4 no components of the product are landfilled.\n\nBenefits and loads beyond the System Boundary (D): Module D includes:\nMaterial recovery potentials from metal recycling and energy recovery potentials from the\nthermal recovery of Packaging.", "lang": "en"}, {"value": "Gültigkeitsbereich: \nDiese EPD bezieht sich auf Holzbauschrauben, Spanplattenschrauben, Bohr- und Blechschrauben, Schrauben für Kunststoffe, metrische Schrauben und stiftförmige Verbindungsmittel mit Gewinde aus Stahl oder Edelstahl. Je nach Schraubentyp werden diese Produkte in der Regel zur Befestigung zweier oder mehrerer Bauteile aus Holz, Stahl oder Kunststoff verwendet. Beispielhafte Anwendungsbereiche sind der Holzbau, Möbel-, Fenster- oder Dachbau sowie Metallleicht- und Stahlbau. Beispielhafte Würth Produktgruppen sind ASSY, Pias und Piasta Schrauben. \nDie deklarierten Umweltdaten, bezogen auf 1 kg Edelstahl, basieren auf einem gewichteten Durchschnitt des Herstellungsprozesses von Edelstahlschrauben in einem Würth-Produktionswerk, zum Beispiel der SWG Schraubenwerk Gaisbach GmbH. Der Inhaber der Deklaration haftet für die zugrundeliegenden Angaben und Nachweise; eine Haftung des IBU (Institut Bauen und Umwelt e. V.) in Bezug auf Herstellerinformationen, Ökobilanzdaten und Nachweise ist ausgeschlossen. Die EPD (Umweltproduktdeklaration) wurde in Übereinstimmung mit der EN 15804 + A2: 2022-03 erstellt. Im Folgenden wird die Norm in vereinfachter Form als EN 15804 bezeichnet. \nSystemgrenze: \nArt der EPD: Cradle-to-Gate - mit Optionen, Modulen C1-C4 und Modul D (A1-A3 + C + D und zusätzliche Module: A4, A5). Produktionsstufe (A1-A3): Die Produktphase umfasst: \n- A1 Rohstoffbeschaffung und -verarbeitung (hauptsächlich Stahl), \n- A2 Transport der Rohstoffe zum Hersteller, \n- A3 Produktion von Edelstahlschrauben (inkl. Energiebereitstellung, Behandlung von Produktionsabfällen, Herstellung von Verpackungsmaterial). \nBauphase (A4-A5): Die Bauphase umfasst: \n- A4 Transport zur Baustelle 100km mit LKW, \n- A5 Entsorgung der Verpackung und Einbau der Edelstahlschraube. \nEnd-of-Life-Phase (C1-C4): Die End-of-Life-Phase umfasst:\n- C1 maschinengestützter Rückbau (Handschrauber; batteriebetrieben) \n- C2 Transport zur Abfallverwertung; 50km mit LKW Die Transportdistanz kann bei Bedarf auf Gebäudeebene angepasst werden (z.B. für 100km tatsächliche Transportdistanz: LCA-Werte mit Faktor 2 multiplizieren) \n- C3 Abfallverwertung zur Wiederverwertung des Edelstahls \n- C4 keine Bestandteile des Produkts werden deponiert. \nNutzen und Lasten jenseits der Systemgrenze (D): Modul D umfasst: Materialrückgewinnungspotenziale durch Metallrecycling und Energierückgewinnungspotenziale durch die thermische Verwertung der Verpackung.", "lang": "de"}], "other": {"anies": [{"name": "referenceToOriginalEPD", "value": {"shortDescription": {"value": "Stainless Steel screws.pdf", "defaultValue": "Stainless Steel screws.pdf", "lstrings": [{"lang": "en", "value": "Stainless Steel screws.pdf"}]}, "type": "source data set", "uuid": {"uuid": "eaae3d35-f5c5-4b7a-9c48-2d57e167547f"}, "refObjectId": "eaae3d35-f5c5-4b7a-9c48-2d57e167547f", "resourceURLs": ["https://oekobaudat.de/OEKOBAU.DAT/resource/sources/eaae3d35-f5c5-4b7a-9c48-2d57e167547f/Stainless_Steel_screws_17993.pdf?version=00.01.000"]}}]}}, "validation": {"review": [{"referenceToNameOfReviewerAndInstitution": [{"shortDescription": [{"value": "Institut Bauen und Umwelt e. V.", "lang": "en"}], "type": "contact data set", "refObjectId": "d111dbec-b024-4be5-86c5-752d6eb2cf95", "uri": "../contacts/d111dbec-b024-4be5-86c5-752d6eb2cf95.xml"}], "type": "Accredited third party review"}]}, "complianceDeclarations": {"compliance": [{"referenceToComplianceSystem": {"shortDescription": [{"value": "DIN EN 15804+A2", "lang": "en"}], "type": "source data set", "refObjectId": "c0016b33-8cf7-415c-ac6e-deba0d21440d", "uri": "../sources/c0016b33-8cf7-415c-ac6e-deba0d21440d.xml"}}, {"referenceToComplianceSystem": {"shortDescription": [{"value": "ISO 14025", "lang": "en"}], "type": "source data set", "refObjectId": "4f2eb655-6e44-4874-a95a-e28f5442cd4d", "uri": "../sources/4f2eb655-6e44-4874-a95a-e28f5442cd4d.xml"}}]}}, "administrativeInformation": {"commissionerAndGoal": {"referenceToCommissioner": [{"shortDescription": [{"value": "Würth Group / Adolf Würth GmbH & Co. KG", "lang": "en"}], "type": "contact data set", "refObjectId": "482e7f46-5590-4715-94f5-6f3abb20168a", "uri": "../contacts/482e7f46-5590-4715-94f5-6f3abb20168a.xml"}]}, "dataGenerator": {"referenceToPersonOrEntityGeneratingTheDataSet": [{"shortDescription": [{"value": "Sphera Solutions GmbH", "lang": "en"}], "type": "contact data set", "refObjectId": "623edf96-39d1-4e6f-9892-674c7228546b", "uri": "../contacts/623edf96-39d1-4e6f-9892-674c7228546b.xml"}]}, "dataEntryBy": {"timeStamp": 1710979200000, "referenceToDataSetFormat": [{"shortDescription": [{"value": "ILCD Format", "lang": "en"}], "type": "source data set", "refObjectId": "a97a0155-0234-4b87-b4ce-a45da52f2a40", "uri": "../sources/a97a0155-0234-4b87-b4ce-a45da52f2a40.xml"}, {"shortDescription": [{"value": "EPD-Datenformaterweiterungen v1.2", "lang": "de"}, {"value": "EPD Data Format Extensions v1.2", "lang": "en"}], "type": "source data set", "refObjectId": "a29449fd-aa2f-4de8-b5d7-4b06b43c6fde", "uri": "../sources/a29449fd-aa2f-4de8-b5d7-4b06b43c6fde.xml"}]}, "publicationAndOwnership": {"dataSetVersion": "00.02.000", "referenceToRegistrationAuthority": {"shortDescription": [{"value": "Institut Bauen und Umwelt e. V.", "lang": "en"}], "type": "contact data set", "refObjectId": "d111dbec-b024-4be5-86c5-752d6eb2cf95", "uri": "../contacts/d111dbec-b024-4be5-86c5-752d6eb2cf95.xml"}, "registrationNumber": "EPD-AWU-20230569-CBA1-EN", "referenceToOwnershipOfDataSet": {"shortDescription": [{"value": "Würth Group / Adolf Würth GmbH & Co. KG", "lang": "en"}], "type": "contact data set", "refObjectId": "482e7f46-5590-4715-94f5-6f3abb20168a", "uri": "../contacts/482e7f46-5590-4715-94f5-6f3abb20168a.xml"}, "copyright": true, "licenseType": "Free of charge for all users and uses", "accessRestrictions": [{"value": "None", "lang": "en"}], "other": {"anies": [{"name": "referenceToPublisher", "value": {"shortDescription": [{"value": "Institut Bauen und Umwelt e. V.", "lang": "en"}], "type": "contact data set", "refObjectId": "d111dbec-b024-4be5-86c5-752d6eb2cf95", "uri": "../contacts/d111dbec-b024-4be5-86c5-752d6eb2cf95.xml"}}]}}}, "exchanges": {"exchange": [{"dataSetInternalID": 0, "referenceToFlowDataSet": {"shortDescription": [{"value": "Stainless steel fasteners with thread (Edelstahlschrauben)", "lang": "en"}], "type": "flow data set", "refObjectId": "a9498f31-0a80-d2e8-0819-389e42110604", "uri": "../flows/a9498f31-0a80-d2e8-0819-389e42110604.xml"}, "meanAmount": 1.0, "referencesToDataSource": {}, "referenceFlow": true, "resolvedFlowVersion": "00.02.000", "resultingflowAmount": 1.0, "flowProperties": [{"name": [{"lang": "en", "value": "Mass"}, {"lang": "de", "value": "Masse"}], "uuid": "93a60a56-a3c8-11da-a746-0800200b9a66", "referenceFlowProperty": true, "meanValue": 1.0, "referenceUnit": "kg", "unitGroupUUID": "ad38d542-3fe9-439d-9b95-2f5f7752acaf"}], "materialProperties": [{"name": "gross density", "value": "1.0", "unit": "kg/m^3", "unitDescription": "kilograms per cubic metre"}], "typeOfFlow": "Product flow", "classification": {"classHierarchy": "Metalle / Edelstahl / Befestigungsmittel", "name": "OEKOBAU.DAT"}}, {"dataSetInternalID": 1, "referenceToFlowDataSet": {"shortDescription": [{"value": "Renewable primary energy as energy carrier (PERE)", "lang": "en"}, {"value": "Erneuerbare Primärenergie als Energieträger (PERE)", "lang": "de"}], "type": "flow data set", "refObjectId": "20f32be5-0398-4288-9b6d-accddd195317", "uri": "../flows/20f32be5-0398-4288-9b6d-accddd195317.xml"}, "exchange direction": "INPUT", "other": {"anies": [{"name": "referenceToUnitGroupDataSet", "value": {"shortDescription": [{"value": "MJ", "lang": "en"}], "type": "unit group data set", "refObjectId": "93a60a57-a3c8-11da-a746-0800200c9a66", "uri": "../unitgroups/93a60a57-a3c8-11da-a746-0800200c9a66.xml"}}, {"value": "13.6667387405361", "module": "A1-A3"}, {"value": "0.00655731592015703", "module": "A4"}, {"value": "0.997489361096939", "module": "A5"}, {"value": "0.128228681864271", "module": "C1"}, {"value": "0.00425799735075132", "module": "C2"}, {"value": "0", "module": "C3"}, {"value": "0", "module": "C4"}, {"value": "-9.94395813337407", "module": "D"}]}, "resolvedFlowVersion": "38.00.000", "flowProperties": [], "typeOfFlow": "Other flow", "classification": {"classHierarchy": "Quantities", "name": "GaBiCategories"}}, {"dataSetInternalID": 2, "referenceToFlowDataSet": {"shortDescription": [{"value": "Renewable primary energy resources as material utilization (PERM)", "lang": "en"}, {"value": "Erneuerbare Primärenergie zur stofflichen Nutzung (PERM)", "lang": "de"}], "type": "flow data set", "refObjectId": "fb3ec0de-548d-4508-aea5-00b73bf6f702", "uri": "../flows/fb3ec0de-548d-4508-aea5-00b73bf6f702.xml"}, "exchange direction": "INPUT", "other": {"anies": [{"name": "referenceToUnitGroupDataSet", "value": {"shortDescription": [{"value": "MJ", "lang": "en"}], "type": "unit group data set", "refObjectId": "93a60a57-a3c8-11da-a746-0800200c9a66", "uri": "../unitgroups/93a60a57-a3c8-11da-a746-0800200c9a66.xml"}}, {"value": "0.864", "module": "A1-A3"}, {"value": "0", "module": "A4"}, {"value": "-0.864", "module": "A5"}, {"value": "0", "module": "C1"}, {"value": "0", "module": "C2"}, {"value": "0", "module": "C3"}, {"value": "0", "module": "C4"}, {"value": "0", "module": "D"}]}, "resolvedFlowVersion": "38.00.000", "flowProperties": [], "typeOfFlow": "Other flow", "classification": {"classHierarchy": "Quantities", "name": "GaBiCategories"}}, {"dataSetInternalID": 3, "referenceToFlowDataSet": {"shortDescription": [{"value": "Total use of renewable primary energy resources (PERT)", "lang": "en"}, {"value": "Total erneuerbare Primärenergie (PERT)", "lang": "de"}], "type": "flow data set", "refObjectId": "53f97275-fa8a-4cdd-9024-65936002acd0", "uri": "../flows/53f97275-fa8a-4cdd-9024-65936002acd0.xml"}, "exchange direction": "INPUT", "other": {"anies": [{"name": "referenceToUnitGroupDataSet", "value": {"shortDescription": [{"value": "MJ", "lang": "en"}], "type": "unit group data set", "refObjectId": "93a60a57-a3c8-11da-a746-0800200c9a66", "uri": "../unitgroups/93a60a57-a3c8-11da-a746-0800200c9a66.xml"}}, {"value": "14.5307387405361", "module": "A1-A3"}, {"value": "0.00655731592015703", "module": "A4"}, {"value": "0.133489361096939", "module": "A5"}, {"value": "0.128228681864271", "module": "C1"}, {"value": "0.00425799735075132", "module": "C2"}, {"value": "0", "module": "C3"}, {"value": "0", "module": "C4"}, {"value": "-9.94395813337407", "module": "D"}]}, "resolvedFlowVersion": "38.00.000", "flowProperties": [], "typeOfFlow": "Other flow", "classification": {"classHierarchy": "Quantities / Environmental quantities / EPD EN 15804 / LCI indicators", "name": "GaBiCategories"}}, {"dataSetInternalID": 4, "referenceToFlowDataSet": {"shortDescription": [{"value": "Non renewable primary energy as energy carrier (PENRE)", "lang": "en"}, {"value": "Nicht-erneuerbare Primärenergie als Energieträger (PENRE)", "lang": "de"}], "type": "flow data set", "refObjectId": "ac857178-2b45-46ec-892a-a9a4332f0372", "uri": "../flows/ac857178-2b45-46ec-892a-a9a4332f0372.xml"}, "exchange direction": "INPUT", "other": {"anies": [{"name": "referenceToUnitGroupDataSet", "value": {"shortDescription": [{"value": "MJ", "lang": "en"}], "type": "unit group data set", "refObjectId": "93a60a57-a3c8-11da-a746-0800200c9a66", "uri": "../unitgroups/93a60a57-a3c8-11da-a746-0800200c9a66.xml"}}, {"value": "74.6065132535389", "module": "A1-A3"}, {"value": "0.0904453977638705", "module": "A4"}, {"value": "0.971693226469198", "module": "A5"}, {"value": "0.936104751532477", "module": "C1"}, {"value": "0.0587307777687471", "module": "C2"}, {"value": "0", "module": "C3"}, {"value": "0", "module": "C4"}, {"value": "-52.7651948357561", "module": "D"}]}, "resolvedFlowVersion": "38.00.000", "flowProperties": [], "typeOfFlow": "Other flow", "classification": {"classHierarchy": "Quantities", "name": "GaBiCategories"}}, {"dataSetInternalID": 5, "referenceToFlowDataSet": {"shortDescription": [{"value": "Non renewable primary energy as material utilization (PENRM)", "lang": "en"}, {"value": "Nicht-erneuerbare Primärenergie zur stofflichen Nutzung (PENRM)", "lang": "de"}], "type": "flow data set", "refObjectId": "1421caa0-679d-4bf4-b282-0eb850ccae27", "uri": "../flows/1421caa0-679d-4bf4-b282-0eb850ccae27.xml"}, "exchange direction": "INPUT", "other": {"anies": [{"name": "referenceToUnitGroupDataSet", "value": {"shortDescription": [{"value": "MJ", "lang": "en"}], "type": "unit group data set", "refObjectId": "93a60a57-a3c8-11da-a746-0800200c9a66", "uri": "../unitgroups/93a60a57-a3c8-11da-a746-0800200c9a66.xml"}}, {"value": "0.0138", "module": "A1-A3"}, {"value": "0", "module": "A4"}, {"value": "-0.0138", "module": "A5"}, {"value": "0", "module": "C1"}, {"value": "0", "module": "C2"}, {"value": "0", "module": "C3"}, {"value": "0", "module": "C4"}, {"value": "0", "module": "D"}]}, "resolvedFlowVersion": "38.00.000", "flowProperties": [], "typeOfFlow": "Other flow", "classification": {"classHierarchy": "Quantities", "name": "GaBiCategories"}}, {"dataSetInternalID": 6, "referenceToFlowDataSet": {"shortDescription": [{"value": "Total use of non renewable primary energy resources (PENRT)", "lang": "en"}, {"value": "Total nicht erneuerbare Primärenergie (PENRT)", "lang": "de"}], "type": "flow data set", "refObjectId": "06159210-646b-4c8d-8583-da9b3b95a6c1", "uri": "../flows/06159210-646b-4c8d-8583-da9b3b95a6c1.xml"}, "exchange direction": "INPUT", "other": {"anies": [{"name": "referenceToUnitGroupDataSet", "value": {"shortDescription": [{"value": "MJ", "lang": "en"}], "type": "unit group data set", "refObjectId": "93a60a57-a3c8-11da-a746-0800200c9a66", "uri": "../unitgroups/93a60a57-a3c8-11da-a746-0800200c9a66.xml"}}, {"value": "74.6203132543177", "module": "A1-A3"}, {"value": "0.0904453977638705", "module": "A4"}, {"value": "0.9578932264692", "module": "A5"}, {"value": "0.936104751532479", "module": "C1"}, {"value": "0.0587307777687471", "module": "C2"}, {"value": "0", "module": "C3"}, {"value": "0", "module": "C4"}, {"value": "-52.7651948376623", "module": "D"}]}, "resolvedFlowVersion": "38.00.000", "flowProperties": [], "typeOfFlow": "Other flow", "classification": {"classHierarchy": "Quantities / Environmental quantities / EPD EN 15804 / LCI indicators", "name": "GaBiCategories"}}, {"dataSetInternalID": 7, "referenceToFlowDataSet": {"shortDescription": [{"value": "Use of secondary material (SM)", "lang": "en"}, {"value": "Einsatz von Sekundärstoffen (SM)", "lang": "de"}], "type": "flow data set", "refObjectId": "c6a1f35f-2d09-4f54-8dfb-97e502e1ce92", "uri": "../flows/c6a1f35f-2d09-4f54-8dfb-97e502e1ce92.xml"}, "exchange direction": "INPUT", "other": {"anies": [{"name": "referenceToUnitGroupDataSet", "value": {"shortDescription": [{"value": "kg", "lang": "en"}], "type": "unit group data set", "refObjectId": "ad38d542-3fe9-439d-9b95-2f5f7752acaf", "uri": "../unitgroups/ad38d542-3fe9-439d-9b95-2f5f7752acaf.xml"}}, {"value": "0.24874896256164", "module": "A1-A3"}, {"value": "0", "module": "A4"}, {"value": "0", "module": "A5"}, {"value": "0", "module": "C1"}, {"value": "0", "module": "C2"}, {"value": "0", "module": "C3"}, {"value": "0", "module": "C4"}, {"value": "0.76125103743836", "module": "D"}]}, "resolvedFlowVersion": "38.00.000", "flowProperties": [], "typeOfFlow": "Other flow", "classification": {"classHierarchy": "Quantities / Environmental quantities / EPD EN 15804 / LCI indicators", "name": "GaBiCategories"}}, {"dataSetInternalID": 8, "referenceToFlowDataSet": {"shortDescription": [{"value": "Use of renewable secondary fuels (RSF)", "lang": "en"}, {"value": "Erneuerbare Sekundärbrennstoffe (RSF)", "lang": "de"}], "type": "flow data set", "refObjectId": "64333088-a55f-4aa2-9a31-c10b07816787", "uri": "../flows/64333088-a55f-4aa2-9a31-c10b07816787.xml"}, "exchange direction": "INPUT", "other": {"anies": [{"name": "referenceToUnitGroupDataSet", "value": {"shortDescription": [{"value": "MJ", "lang": "en"}], "type": "unit group data set", "refObjectId": "93a60a57-a3c8-11da-a746-0800200c9a66", "uri": "../unitgroups/93a60a57-a3c8-11da-a746-0800200c9a66.xml"}}, {"value": "0", "module": "A1-A3"}, {"value": "0", "module": "A4"}, {"value": "0", "module": "A5"}, {"value": "0", "module": "C1"}, {"value": "0", "module": "C2"}, {"value": "0", "module": "C3"}, {"value": "0", "module": "C4"}, {"value": "0", "module": "D"}]}, "resolvedFlowVersion": "38.00.000", "flowProperties": [], "typeOfFlow": "Other flow", "classification": {"classHierarchy": "Quantities / Environmental quantities / EPD EN 15804 / LCI indicators", "name": "GaBiCategories"}}, {"dataSetInternalID": 9, "referenceToFlowDataSet": {"shortDescription": [{"value": "Use of non renewable secondary fuels (NRSF)", "lang": "en"}, {"value": "Nicht erneuerbare Sekundärbrennstoffe (NRSF)", "lang": "de"}], "type": "flow data set", "refObjectId": "89def144-d39a-4287-b86f-efde453ddcb2", "uri": "../flows/89def144-d39a-4287-b86f-efde453ddcb2.xml"}, "exchange direction": "INPUT", "other": {"anies": [{"name": "referenceToUnitGroupDataSet", "value": {"shortDescription": [{"value": "MJ", "lang": "en"}], "type": "unit group data set", "refObjectId": "93a60a57-a3c8-11da-a746-0800200c9a66", "uri": "../unitgroups/93a60a57-a3c8-11da-a746-0800200c9a66.xml"}}, {"value": "0", "module": "A1-A3"}, {"value": "0", "module": "A4"}, {"value": "0", "module": "A5"}, {"value": "0", "module": "C1"}, {"value": "0", "module": "C2"}, {"value": "0", "module": "C3"}, {"value": "0", "module": "C4"}, {"value": "0", "module": "D"}]}, "resolvedFlowVersion": "38.00.000", "flowProperties": [], "typeOfFlow": "Other flow", "classification": {"classHierarchy": "Quantities / Environmental quantities / EPD EN 15804 / LCI indicators", "name": "GaBiCategories"}}, {"dataSetInternalID": 10, "referenceToFlowDataSet": {"shortDescription": [{"value": "Use of net fresh water (FW)", "lang": "en"}, {"value": "Einsatz von Süßwasserressourcen (FW)", "lang": "de"}], "type": "flow data set", "refObjectId": "3cf952c8-f3a4-461d-8c96-96456ca62246", "uri": "../flows/3cf952c8-f3a4-461d-8c96-96456ca62246.xml"}, "exchange direction": "INPUT", "other": {"anies": [{"name": "referenceToUnitGroupDataSet", "value": {"shortDescription": [{"value": "m^3", "lang": "en"}], "type": "unit group data set", "refObjectId": "cd950537-0a98-4044-9ba7-9f9a68d0a504", "uri": "../unitgroups/cd950537-0a98-4044-9ba7-9f9a68d0a504.xml"}}, {"value": "0.0819062210290217", "module": "A1-A3"}, {"value": "7.18202824174965E-06", "module": "A4"}, {"value": "0.000414630911621319", "module": "A5"}, {"value": "0.000214588030886378", "module": "C1"}, {"value": "4.66365470243481E-06", "module": "C2"}, {"value": "0", "module": "C3"}, {"value": "0", "module": "C4"}, {"value": "-0.0717251207716298", "module": "D"}]}, "resolvedFlowVersion": "38.00.000", "flowProperties": [], "typeOfFlow": "Other flow", "classification": {"classHierarchy": "Quantities / Environmental quantities / EPD EN 15804 / LCI indicators", "name": "GaBiCategories"}}, {"dataSetInternalID": 11, "referenceToFlowDataSet": {"shortDescription": [{"value": "Hazardous waste disposed (HWD)", "lang": "en"}, {"value": "Gefährlicher Abfall zur Deponie (HWD)", "lang": "de"}], "type": "flow data set", "refObjectId": "430f9e0f-59b2-46a0-8e0d-55e0e84948fc", "uri": "../flows/430f9e0f-59b2-46a0-8e0d-55e0e84948fc.xml"}, "exchange direction": "OUTPUT", "other": {"anies": [{"name": "referenceToUnitGroupDataSet", "value": {"shortDescription": [{"value": "kg", "lang": "en"}], "type": "unit group data set", "refObjectId": "ad38d542-3fe9-439d-9b95-2f5f7752acaf", "uri": "../unitgroups/ad38d542-3fe9-439d-9b95-2f5f7752acaf.xml"}}, {"value": "1.75948409669568E-06", "module": "A1-A3"}, {"value": "2.80047654389017E-13", "module": "A4"}, {"value": "5.49390187016945E-11", "module": "A5"}, {"value": "5.42582850447365E-11", "module": "C1"}, {"value": "1.81849126226635E-13", "module": "C2"}, {"value": "0", "module": "C3"}, {"value": "0", "module": "C4"}, {"value": "-0.000480155237509252", "module": "D"}]}, "resolvedFlowVersion": "38.00.000", "flowProperties": [], "typeOfFlow": "Other flow", "classification": {"classHierarchy": "Quantities / Environmental quantities / EPD EN 15804 / LCI indicators", "name": "GaBiCategories"}}, {"dataSetInternalID": 12, "referenceToFlowDataSet": {"shortDescription": [{"value": "Non hazardous waste disposed (NHWD)", "lang": "en"}, {"value": "Entsorgter nicht gefährlicher Abfall (NHWD)", "lang": "de"}], "type": "flow data set", "refObjectId": "b29ef66b-e286-4afa-949f-62f1a7b4d7fa", "uri": "../flows/b29ef66b-e286-4afa-949f-62f1a7b4d7fa.xml"}, "exchange direction": "OUTPUT", "other": {"anies": [{"name": "referenceToUnitGroupDataSet", "value": {"shortDescription": [{"value": "kg", "lang": "en"}], "type": "unit group data set", "refObjectId": "ad38d542-3fe9-439d-9b95-2f5f7752acaf", "uri": "../unitgroups/ad38d542-3fe9-439d-9b95-2f5f7752acaf.xml"}}, {"value": "3.65431258998894", "module": "A1-A3"}, {"value": "1.37874193967322E-05", "module": "A4"}, {"value": "0.00241113104671072", "module": "A5"}, {"value": "0.000206347174487487", "module": "C1"}, {"value": "8.9528697381378E-06", "module": "C2"}, {"value": "0", "module": "C3"}, {"value": "0", "module": "C4"}, {"value": "0.0468287675678285", "module": "D"}]}, "resolvedFlowVersion": "38.00.000", "flowProperties": [], "typeOfFlow": "Other flow", "classification": {"classHierarchy": "Quantities / Environmental quantities / EPD EN 15804 / LCI indicators", "name": "GaBiCategories"}}, {"dataSetInternalID": 13, "referenceToFlowDataSet": {"shortDescription": [{"value": "Radioactive waste disposed (RWD)", "lang": "en"}, {"value": "Entsorgter radioaktiver Abfall (RWD)", "lang": "de"}], "type": "flow data set", "refObjectId": "3449546e-52ad-4b39-b809-9fb77cea8ff6", "uri": "../flows/3449546e-52ad-4b39-b809-9fb77cea8ff6.xml"}, "exchange direction": "OUTPUT", "other": {"anies": [{"name": "referenceToUnitGroupDataSet", "value": {"shortDescription": [{"value": "kg", "lang": "en"}], "type": "unit group data set", "refObjectId": "ad38d542-3fe9-439d-9b95-2f5f7752acaf", "uri": "../unitgroups/ad38d542-3fe9-439d-9b95-2f5f7752acaf.xml"}}, {"value": "0.0010799062817953", "module": "A1-A3"}, {"value": "1.69263182377516E-07", "module": "A4"}, {"value": "0.000146974220406712", "module": "A5"}, {"value": "0.000145824466761776", "module": "C1"}, {"value": "1.09911157387997E-07", "module": "C2"}, {"value": "0", "module": "C3"}, {"value": "0", "module": "C4"}, {"value": "-0.000372728929569031", "module": "D"}]}, "resolvedFlowVersion": "38.00.000", "flowProperties": [], "typeOfFlow": "Other flow", "classification": {"classHierarchy": "Quantities / Environmental quantities / EPD EN 15804 / LCI indicators", "name": "GaBiCategories"}}, {"dataSetInternalID": 14, "referenceToFlowDataSet": {"shortDescription": [{"value": "Components for re-use (CRU)", "lang": "en"}, {"value": "Komponenten für die Wiederverwendung (CRU)", "lang": "de"}], "type": "flow data set", "refObjectId": "a2b32f97-3fc7-4af2-b209-525bc6426f33", "uri": "../flows/a2b32f97-3fc7-4af2-b209-525bc6426f33.xml"}, "exchange direction": "OUTPUT", "other": {"anies": [{"name": "referenceToUnitGroupDataSet", "value": {"shortDescription": [{"value": "kg", "lang": "en"}], "type": "unit group data set", "refObjectId": "ad38d542-3fe9-439d-9b95-2f5f7752acaf", "uri": "../unitgroups/ad38d542-3fe9-439d-9b95-2f5f7752acaf.xml"}}, {"value": "0", "module": "A1-A3"}, {"value": "0", "module": "A4"}, {"value": "0", "module": "A5"}, {"value": "0", "module": "C1"}, {"value": "0", "module": "C2"}, {"value": "0", "module": "C3"}, {"value": "0", "module": "C4"}, {"value": "0", "module": "D"}]}, "resolvedFlowVersion": "38.00.000", "flowProperties": [], "typeOfFlow": "Other flow", "classification": {"classHierarchy": "Quantities / Environmental quantities / EPD EN 15804 / LCI indicators", "name": "GaBiCategories"}}, {"dataSetInternalID": 15, "referenceToFlowDataSet": {"shortDescription": [{"value": "Materials for recycling (MFR)", "lang": "en"}, {"value": "Stoffe zum Recycling (MFR)", "lang": "de"}], "type": "flow data set", "refObjectId": "d7fe48a5-4103-49c8-9aae-b0b5dfdbd6ae", "uri": "../flows/d7fe48a5-4103-49c8-9aae-b0b5dfdbd6ae.xml"}, "exchange direction": "OUTPUT", "other": {"anies": [{"name": "referenceToUnitGroupDataSet", "value": {"shortDescription": [{"value": "kg", "lang": "en"}], "type": "unit group data set", "refObjectId": "ad38d542-3fe9-439d-9b95-2f5f7752acaf", "uri": "../unitgroups/ad38d542-3fe9-439d-9b95-2f5f7752acaf.xml"}}, {"value": "0.0102020201", "module": "A1-A3"}, {"value": "0", "module": "A4"}, {"value": "0", "module": "A5"}, {"value": "0", "module": "C1"}, {"value": "0", "module": "C2"}, {"value": "0.9997979799", "module": "C3"}, {"value": "0", "module": "C4"}, {"value": "0", "module": "D"}]}, "resolvedFlowVersion": "38.00.000", "flowProperties": [], "typeOfFlow": "Other flow", "classification": {"classHierarchy": "Quantities / Environmental quantities / EPD EN 15804 / LCI indicators", "name": "GaBiCategories"}}, {"dataSetInternalID": 16, "referenceToFlowDataSet": {"shortDescription": [{"value": "Materials for energy recovery (MER)", "lang": "en"}, {"value": "Stoffe für die Energierückgewinnung (MER)", "lang": "de"}], "type": "flow data set", "refObjectId": "59a9181c-3aaf-46ee-8b13-2b3723b6e447", "uri": "../flows/59a9181c-3aaf-46ee-8b13-2b3723b6e447.xml"}, "exchange direction": "OUTPUT", "other": {"anies": [{"name": "referenceToUnitGroupDataSet", "value": {"shortDescription": [{"value": "kg", "lang": "en"}], "type": "unit group data set", "refObjectId": "ad38d542-3fe9-439d-9b95-2f5f7752acaf", "uri": "../unitgroups/ad38d542-3fe9-439d-9b95-2f5f7752acaf.xml"}}, {"value": "0", "module": "A1-A3"}, {"value": "0", "module": "A4"}, {"value": "0", "module": "A5"}, {"value": "0", "module": "C1"}, {"value": "0", "module": "C2"}, {"value": "0", "module": "C3"}, {"value": "0", "module": "C4"}, {"value": "0", "module": "D"}]}, "resolvedFlowVersion": "38.00.000", "flowProperties": [], "typeOfFlow": "Other flow", "classification": {"classHierarchy": "Quantities / Environmental quantities / EPD EN 15804 / LCI indicators", "name": "GaBiCategories"}}, {"dataSetInternalID": 17, "referenceToFlowDataSet": {"shortDescription": [{"value": "Exported electrical energy (EEE)", "lang": "en"}, {"value": "Exportierte elektrische Energie (EEE)", "lang": "de"}], "type": "flow data set", "refObjectId": "4da0c987-2b76-40d6-9e9e-82a017aaaf29", "uri": "../flows/4da0c987-2b76-40d6-9e9e-82a017aaaf29.xml"}, "exchange direction": "OUTPUT", "other": {"anies": [{"name": "referenceToUnitGroupDataSet", "value": {"shortDescription": [{"value": "MJ", "lang": "en"}], "type": "unit group data set", "refObjectId": "93a60a57-a3c8-11da-a746-0800200c9a66", "uri": "../unitgroups/93a60a57-a3c8-11da-a746-0800200c9a66.xml"}}, {"value": "0", "module": "A1-A3"}, {"value": "0", "module": "A4"}, {"value": "0.10431984561931", "module": "A5"}, {"value": "0", "module": "C1"}, {"value": "0", "module": "C2"}, {"value": "0", "module": "C3"}, {"value": "0", "module": "C4"}, {"value": "0", "module": "D"}]}, "resolvedFlowVersion": "38.00.000", "flowProperties": [], "typeOfFlow": "Other flow", "classification": {"classHierarchy": "Quantities / Environmental quantities / EPD EN 15804 / LCI indicators", "name": "GaBiCategories"}}, {"dataSetInternalID": 18, "referenceToFlowDataSet": {"shortDescription": [{"value": "Exported thermal energy (EET)", "lang": "en"}, {"value": "Exportierte thermische Energie (EET)", "lang": "de"}], "type": "flow data set", "refObjectId": "98daf38a-7a79-46d3-9a37-2b7bd0955810", "uri": "../flows/98daf38a-7a79-46d3-9a37-2b7bd0955810.xml"}, "exchange direction": "OUTPUT", "other": {"anies": [{"name": "referenceToUnitGroupDataSet", "value": {"shortDescription": [{"value": "MJ", "lang": "en"}], "type": "unit group data set", "refObjectId": "93a60a57-a3c8-11da-a746-0800200c9a66", "uri": "../unitgroups/93a60a57-a3c8-11da-a746-0800200c9a66.xml"}}, {"value": "0", "module": "A1-A3"}, {"value": "0", "module": "A4"}, {"value": "0.189163885219834", "module": "A5"}, {"value": "0", "module": "C1"}, {"value": "0", "module": "C2"}, {"value": "0", "module": "C3"}, {"value": "0", "module": "C4"}, {"value": "0", "module": "D"}]}, "resolvedFlowVersion": "38.00.000", "flowProperties": [], "typeOfFlow": "Other flow", "classification": {"classHierarchy": "Quantities / Environmental quantities / EPD EN 15804 / LCI indicators", "name": "GaBiCategories"}}]}, "LCIAResults": {"LCIAResult": [{"referenceToLCIAMethodDataSet": {"shortDescription": [{"value": "Global Warming Potential total (GWP-total)", "lang": "en"}, {"value": "Globales Erwärmungspotenzial total (GWP-total)", "lang": "de"}], "type": "LCIA method data set", "refObjectId": "6a37f984-a4b3-458a-a20a-64418c145fa2", "uri": "../lciamethods/6a37f984-a4b3-458a-a20a-64418c145fa2.xml"}, "other": {"anies": [{"name": "referenceToUnitGroupDataSet", "value": {"shortDescription": [{"value": "kg CO_(2) eq", "lang": "en"}], "type": "unit group data set", "refObjectId": "1ebf3012-d0db-4de2-aefd-ef30cedb0be1", "uri": "../unitgroups/1ebf3012-d0db-4de2-aefd-ef30cedb0be1.xml"}}, {"value": "6.88346076619204", "module": "A1-A3"}, {"value": "0.00668847095513505", "module": "A4"}, {"value": "0.120465883541386", "module": "A5"}, {"value": "0.0426362349922894", "module": "C1"}, {"value": "0.0043431629578799", "module": "C2"}, {"value": "0", "module": "C3"}, {"value": "0", "module": "C4"}, {"value": "-4.31283111139019", "module": "D"}]}}, {"referenceToLCIAMethodDataSet": {"shortDescription": [{"value": "Global Warming Potential fossil fuels (GWP-fossil)", "lang": "en"}, {"value": "Globales Erwärmungspotenzial fossil (GWP-fossil)", "lang": "de"}], "type": "LCIA method data set", "refObjectId": "5f635281-343e-44fb-83df-1971b155e6b6", "uri": "../lciamethods/5f635281-343e-44fb-83df-1971b155e6b6.xml"}, "other": {"anies": [{"name": "referenceToUnitGroupDataSet", "value": {"shortDescription": [{"value": "kg CO_(2) eq", "lang": "en"}], "type": "unit group data set", "refObjectId": "1ebf3012-d0db-4de2-aefd-ef30cedb0be1", "uri": "../unitgroups/1ebf3012-d0db-4de2-aefd-ef30cedb0be1.xml"}}, {"value": "6.9426476496803", "module": "A1-A3"}, {"value": "0.00660767962602898", "module": "A4"}, {"value": "0.0449673449016945", "module": "A5"}, {"value": "0.0426111265296663", "module": "C1"}, {"value": "0.00429070105586297", "module": "C2"}, {"value": "0", "module": "C3"}, {"value": "0", "module": "C4"}, {"value": "-4.32122479635103", "module": "D"}]}}, {"referenceToLCIAMethodDataSet": {"shortDescription": [{"value": "Global Warming Potential biogenic (GWP-biogenic)", "lang": "en"}, {"value": "Globales Erwärmungspotenzial biogen (GWP-biogenic)", "lang": "de"}], "type": "LCIA method data set", "refObjectId": "2356e1ab-0185-4db5-86e5-16de51c7485c", "uri": "../lciamethods/2356e1ab-0185-4db5-86e5-16de51c7485c.xml"}, "other": {"anies": [{"name": "referenceToUnitGroupDataSet", "value": {"shortDescription": [{"value": "kg CO_(2) eq", "lang": "en"}], "type": "unit group data set", "refObjectId": "1ebf3012-d0db-4de2-aefd-ef30cedb0be1", "uri": "../unitgroups/1ebf3012-d0db-4de2-aefd-ef30cedb0be1.xml"}}, {"value": "-0.0743529526041631", "module": "A1-A3"}, {"value": "1.9532543912313E-05", "module": "A4"}, {"value": "0.0754942516981415", "module": "A5"}, {"value": "2.12110466857899E-05", "module": "C1"}, {"value": "1.26834700729305E-05", "module": "C2"}, {"value": "0", "module": "C3"}, {"value": "0", "module": "C4"}, {"value": "0.019805068500322", "module": "D"}]}}, {"referenceToLCIAMethodDataSet": {"shortDescription": [{"value": "Global Warming Potential luluc (GWP-luluc)", "lang": "en"}, {"value": "Globales Erwärmungspotenzial luluc (GWP-luluc)", "lang": "de"}], "type": "LCIA method data set", "refObjectId": "4331bbdb-978a-490d-8707-eeb047f01a55", "uri": "../lciamethods/4331bbdb-978a-490d-8707-eeb047f01a55.xml"}, "other": {"anies": [{"name": "referenceToUnitGroupDataSet", "value": {"shortDescription": [{"value": "kg CO_(2) eq", "lang": "en"}], "type": "unit group data set", "refObjectId": "1ebf3012-d0db-4de2-aefd-ef30cedb0be1", "uri": "../unitgroups/1ebf3012-d0db-4de2-aefd-ef30cedb0be1.xml"}}, {"value": "0.0151660691158975", "module": "A1-A3"}, {"value": "6.12587851937546E-05", "module": "A4"}, {"value": "4.28694154984943E-06", "module": "A5"}, {"value": "3.89741593731769E-06", "module": "C1"}, {"value": "3.97784319439965E-05", "module": "C2"}, {"value": "0", "module": "C3"}, {"value": "0", "module": "C4"}, {"value": "-0.011411383539482", "module": "D"}]}}, {"referenceToLCIAMethodDataSet": {"shortDescription": [{"value": "Depletion potential of the stratospheric ozone layer (ODP)", "lang": "en"}, {"value": "Abbau Potential der stratosphärischen Ozonschicht (ODP)", "lang": "de"}], "type": "LCIA method data set", "refObjectId": "b5c629d6-def3-11e6-bf01-fe55135034f3", "uri": "../lciamethods/b5c629d6-def3-11e6-bf01-fe55135034f3.xml"}, "other": {"anies": [{"name": "referenceToUnitGroupDataSet", "value": {"shortDescription": [{"value": "kg CFC11 eq", "lang": "en"}], "type": "unit group data set", "refObjectId": "d9e957c9-7309-4474-bf3a-7777df6c4e5b", "uri": "../unitgroups/d9e957c9-7309-4474-bf3a-7777df6c4e5b.xml"}}, {"value": "6.76038215939622E-12", "module": "A1-A3"}, {"value": "8.60644930127025E-16", "module": "A4"}, {"value": "4.27500272288007E-13", "module": "A5"}, {"value": "4.19028705067606E-13", "module": "C1"}, {"value": "5.58860344238328E-16", "module": "C2"}, {"value": "0", "module": "C3"}, {"value": "0", "module": "C4"}, {"value": "-1.75736257395091E-13", "module": "D"}]}}, {"referenceToLCIAMethodDataSet": {"shortDescription": [{"value": "Acidification potential of land and water (AP)", "lang": "en"}, {"value": "Versauerungspotenzial von Boden und Wasser (AP)", "lang": "de"}], "type": "LCIA method data set", "refObjectId": "b5c611c6-def3-11e6-bf01-fe55135034f3", "uri": "../lciamethods/b5c611c6-def3-11e6-bf01-fe55135034f3.xml"}, "other": {"anies": [{"name": "referenceToUnitGroupDataSet", "value": {"shortDescription": [{"value": "mol H^(+) eq", "lang": "en"}], "type": "unit group data set", "refObjectId": "42e089ac-92bf-4bf2-8ca1-5fc40d18f2ed", "uri": "../unitgroups/42e089ac-92bf-4bf2-8ca1-5fc40d18f2ed.xml"}}, {"value": "0.0391581703556525", "module": "A1-A3"}, {"value": "9.860193643666E-06", "module": "A4"}, {"value": "8.37274557995693E-05", "module": "A5"}, {"value": "6.48954903091181E-05", "module": "C1"}, {"value": "6.40272314523766E-06", "module": "C2"}, {"value": "0", "module": "C3"}, {"value": "0", "module": "C4"}, {"value": "-0.0262806973317283", "module": "D"}]}}, {"referenceToLCIAMethodDataSet": {"shortDescription": [{"value": "Eutrophication potential aquatic freshwater (EP-freshwater)", "lang": "en"}, {"value": "Eutrophierungspotenzial Süßwasser (EP-freshwater)", "lang": "de"}], "type": "LCIA method data set", "refObjectId": "b53ec18f-7377-4ad3-86eb-cc3f4f276b2b", "uri": "../lciamethods/b53ec18f-7377-4ad3-86eb-cc3f4f276b2b.xml"}, "other": {"anies": [{"name": "referenceToUnitGroupDataSet", "value": {"shortDescription": [{"value": "kg P eq", "lang": "en"}], "type": "unit group data set", "refObjectId": "0429039d-a61d-4590-ba67-aa4a20a810a1", "uri": "../unitgroups/0429039d-a61d-4590-ba67-aa4a20a810a1.xml"}}, {"value": "1.43030600008049E-05", "module": "A1-A3"}, {"value": "2.41829346893589E-08", "module": "A4"}, {"value": "4.47682745297794E-08", "module": "A5"}, {"value": "4.21224788845624E-08", "module": "C1"}, {"value": "1.57032043437395E-08", "module": "C2"}, {"value": "0", "module": "C3"}, {"value": "0", "module": "C4"}, {"value": "-6.21047963687953E-06", "module": "D"}]}}, {"referenceToLCIAMethodDataSet": {"shortDescription": [{"value": "Eutrophication potential aquatic marine (EP-marine)", "lang": "en"}, {"value": "Eutrophierungspotenzial Salzwasser (EP-marine)", "lang": "de"}], "type": "LCIA method data set", "refObjectId": "b5c619fa-def3-11e6-bf01-fe55135034f3", "uri": "../lciamethods/b5c619fa-def3-11e6-bf01-fe55135034f3.xml"}, "other": {"anies": [{"name": "referenceToUnitGroupDataSet", "value": {"shortDescription": [{"value": "kg N eq", "lang": "en"}], "type": "unit group data set", "refObjectId": "d05bb823-ecdf-4686-8c40-bf1d9257859f", "uri": "../unitgroups/d05bb823-ecdf-4686-8c40-bf1d9257859f.xml"}}, {"value": "0.00688144869864296", "module": "A1-A3"}, {"value": "3.59603332810757E-06", "module": "A4"}, {"value": "2.51503915577511E-05", "module": "A5"}, {"value": "1.82971225511634E-05", "module": "C1"}, {"value": "2.33508657669323E-06", "module": "C2"}, {"value": "0", "module": "C3"}, {"value": "0", "module": "C4"}, {"value": "-0.00377877984058221", "module": "D"}]}}, {"referenceToLCIAMethodDataSet": {"shortDescription": [{"value": "Eutrophication potential terrestrial (EP-terrestrial)", "lang": "en"}, {"value": "Eutrophierungspotenzial Land (EP-terrestrial)", "lang": "de"}], "type": "LCIA method data set", "refObjectId": "b5c614d2-def3-11e6-bf01-fe55135034f3", "uri": "../lciamethods/b5c614d2-def3-11e6-bf01-fe55135034f3.xml"}, "other": {"anies": [{"name": "referenceToUnitGroupDataSet", "value": {"shortDescription": [{"value": "mol N eq", "lang": "en"}], "type": "unit group data set", "refObjectId": "71b4d617-0ec9-4d3f-b65e-e438940c2401", "uri": "../unitgroups/71b4d617-0ec9-4d3f-b65e-e438940c2401.xml"}}, {"value": "0.0745868445498471", "module": "A1-A3"}, {"value": "4.25086475289087E-05", "module": "A4"}, {"value": "0.000278912887367283", "module": "A5"}, {"value": "0.000193277948605724", "module": "C1"}, {"value": "2.76030178759147E-05", "module": "C2"}, {"value": "0", "module": "C3"}, {"value": "0", "module": "C4"}, {"value": "-0.0409362558602555", "module": "D"}]}}, {"referenceToLCIAMethodDataSet": {"shortDescription": [{"value": "Formation potential of tropospheric ozone photochemical oxidants (POCP)", "lang": "en"}, {"value": "Bildungspotential für troposphärisches Ozon (POCP)", "lang": "de"}], "type": "LCIA method data set", "refObjectId": "b5c610fe-def3-11e6-bf01-fe55135034f3", "uri": "../lciamethods/b5c610fe-def3-11e6-bf01-fe55135034f3.xml"}, "other": {"anies": [{"name": "referenceToUnitGroupDataSet", "value": {"shortDescription": [{"value": "kg NMVOC eq", "lang": "en"}], "type": "unit group data set", "refObjectId": "d27c25f8-fbc1-44c6-b47b-4adbae4199c6", "uri": "../unitgroups/d27c25f8-fbc1-44c6-b47b-4adbae4199c6.xml"}}, {"value": "0.0198973138032651", "module": "A1-A3"}, {"value": "8.65717020565086E-06", "module": "A4"}, {"value": "6.87070141248526E-05", "module": "A5"}, {"value": "5.05698300696964E-05", "module": "C1"}, {"value": "5.62153909457848E-06", "module": "C2"}, {"value": "0", "module": "C3"}, {"value": "0", "module": "C4"}, {"value": "-0.0114992223003511", "module": "D"}]}}, {"referenceToLCIAMethodDataSet": {"shortDescription": [{"value": "Abiotic depletion potential for non fossil resources (ADPE)", "lang": "en"}, {"value": "Potenzial für den abiotischen Abbau nicht fossiler Ressourcen (ADPE)", "lang": "de"}], "type": "LCIA method data set", "refObjectId": "b2ad6494-c78d-11e6-9d9d-cec0c932ce01", "uri": "../lciamethods/b2ad6494-c78d-11e6-9d9d-cec0c932ce01.xml"}, "other": {"anies": [{"name": "referenceToUnitGroupDataSet", "value": {"shortDescription": [{"value": "kg Sb eq", "lang": "en"}], "type": "unit group data set", "refObjectId": "54ccd2d9-a32a-4fc2-923d-f2c8c93e89d4", "uri": "../unitgroups/54ccd2d9-a32a-4fc2-923d-f2c8c93e89d4.xml"}}, {"value": "0.000233841321451933", "module": "A1-A3"}, {"value": "4.35607847048093E-10", "module": "A4"}, {"value": "2.14089293117016E-09", "module": "A5"}, {"value": "2.06367011622505E-09", "module": "C1"}, {"value": "2.82862238342917E-10", "module": "C2"}, {"value": "0", "module": "C3"}, {"value": "0", "module": "C4"}, {"value": "-6.29756440153046E-06", "module": "D"}]}}, {"referenceToLCIAMethodDataSet": {"shortDescription": [{"value": "Abiotic depletion potential for fossil resources (ADPF)", "lang": "en"}, {"value": "Potenzial für den abiotischen Abbau fossiler Brennstoffe (ADPF)", "lang": "de"}], "type": "LCIA method data set", "refObjectId": "b2ad6110-c78d-11e6-9d9d-cec0c932ce01", "uri": "../lciamethods/b2ad6110-c78d-11e6-9d9d-cec0c932ce01.xml"}, "other": {"anies": [{"name": "referenceToUnitGroupDataSet", "value": {"shortDescription": [{"value": "MJ", "lang": "en"}], "type": "unit group data set", "refObjectId": "93a60a57-a3c8-11da-a746-0800200c9a66", "uri": "../unitgroups/93a60a57-a3c8-11da-a746-0800200c9a66.xml"}}, {"value": "74.4983222085721", "module": "A1-A3"}, {"value": "0.0901045033670637", "module": "A4"}, {"value": "0.957712675466648", "module": "A5"}, {"value": "0.935939086406561", "module": "C1"}, {"value": "0.0585094177708206", "module": "C2"}, {"value": "0", "module": "C3"}, {"value": "0", "module": "C4"}, {"value": "-52.7322909875927", "module": "D"}]}}, {"referenceToLCIAMethodDataSet": {"shortDescription": [{"value": "Water use (WDP)", "lang": "en"}, {"value": "Wassernutzung (WDP)", "lang": "de"}], "type": "LCIA method data set", "refObjectId": "b2ad66ce-c78d-11e6-9d9d-cec0c932ce01", "uri": "../lciamethods/b2ad66ce-c78d-11e6-9d9d-cec0c932ce01.xml"}, "other": {"anies": [{"name": "referenceToUnitGroupDataSet", "value": {"shortDescription": [{"value": "m^(3) world eq deprived", "lang": "en"}], "type": "unit group data set", "refObjectId": "6ae2df01-888e-46c8-b17d-49fa3869b476", "uri": "../unitgroups/6ae2df01-888e-46c8-b17d-49fa3869b476.xml"}}, {"value": "2.25588120122102", "module": "A1-A3"}, {"value": "7.9926697058386E-05", "module": "A4"}, {"value": "0.0120769108360929", "module": "A5"}, {"value": "0.00358084371501766", "module": "C1"}, {"value": "5.19004526353182E-05", "module": "C2"}, {"value": "0", "module": "C3"}, {"value": "0", "module": "C4"}, {"value": "-1.74921375608693", "module": "D"}]}}, {"referenceToLCIAMethodDataSet": {"shortDescription": [{"value": "Incidence of disease due to PM emissions (PM)", "lang": "en"}, {"value": "Auftreten von Krankheiten aufgrund von Feinstaubemissionen (PM)", "lang": "de"}], "type": "LCIA method data set", "refObjectId": "b5c602c6-def3-11e6-bf01-fe55135034f3", "uri": "../lciamethods/b5c602c6-def3-11e6-bf01-fe55135034f3.xml"}, "other": {"anies": [{"name": "referenceToUnitGroupDataSet", "value": {"shortDescription": [{"value": "Disease incidence", "lang": "en"}], "type": "unit group data set", "refObjectId": "3883559b-648f-4afc-8ba2-0bd24f3affa3", "uri": "../unitgroups/3883559b-648f-4afc-8ba2-0bd24f3affa3.xml"}}, {"value": "6.13029751662735E-07", "module": "A1-A3"}, {"value": "8.16357431530247E-11", "module": "A4"}, {"value": "6.90274410481643E-10", "module": "A5"}, {"value": "5.86716793118436E-10", "module": "C1"}, {"value": "5.30102228266394E-11", "module": "C2"}, {"value": "0", "module": "C3"}, {"value": "0", "module": "C4"}, {"value": "-5.68101015540524E-07", "module": "D"}]}}, {"referenceToLCIAMethodDataSet": {"shortDescription": [{"value": "Human exposure efficiency relative to U235 (IR)", "lang": "en"}, {"value": "Wirkung durch Exposition des Menschen mit U235 (IR)", "lang": "de"}], "type": "LCIA method data set", "refObjectId": "b5c632be-def3-11e6-bf01-fe55135034f3", "uri": "../lciamethods/b5c632be-def3-11e6-bf01-fe55135034f3.xml"}, "other": {"anies": [{"name": "referenceToUnitGroupDataSet", "value": {"shortDescription": [{"value": "kBq U235 eq", "lang": "en"}], "type": "unit group data set", "refObjectId": "456b05bf-1415-44a9-9993-02452f554c09", "uri": "../unitgroups/456b05bf-1415-44a9-9993-02452f554c09.xml"}}, {"value": "0.110259963079959", "module": "A1-A3"}, {"value": "2.52415398975387E-05", "module": "A4"}, {"value": "0.0220777186051149", "module": "A5"}, {"value": "0.0218956149998376", "module": "C1"}, {"value": "1.63906103230771E-05", "module": "C2"}, {"value": "0", "module": "C3"}, {"value": "0", "module": "C4"}, {"value": "-0.0418706242517467", "module": "D"}]}}, {"referenceToLCIAMethodDataSet": {"shortDescription": [{"value": "Comparative toxic unit for ecosystems (ETP-fw)", "lang": "en"}, {"value": "Toxizitätsvergleichseinheit für Ökosysteme (ETP-fw)", "lang": "de"}], "type": "LCIA method data set", "refObjectId": "ee1082d1-b0f7-43ca-a1f0-21e2a4a74511", "uri": "../lciamethods/ee1082d1-b0f7-43ca-a1f0-21e2a4a74511.xml"}, "other": {"anies": [{"name": "referenceToUnitGroupDataSet", "value": {"shortDescription": [{"value": "CTUe", "lang": "en"}], "type": "unit group data set", "refObjectId": "aa959ded-f1eb-4efb-9c5c-2d60be36b3e6", "uri": "../unitgroups/aa959ded-f1eb-4efb-9c5c-2d60be36b3e6.xml"}}, {"value": "23.1953758519434", "module": "A1-A3"}, {"value": "0.0639974187615064", "module": "A4"}, {"value": "0.278338392367761", "module": "A5"}, {"value": "0.268072419069461", "module": "C1"}, {"value": "0.0415567654295496", "module": "C2"}, {"value": "0", "module": "C3"}, {"value": "0", "module": "C4"}, {"value": "-31.5035024792867", "module": "D"}]}}, {"referenceToLCIAMethodDataSet": {"shortDescription": [{"value": "Comparative toxic unit for humans (carcinogenic) (HTP-c)", "lang": "en"}, {"value": "Toxizitätsvergleichseinheit für Menschen (krebserregend) (HTP-c)", "lang": "de"}], "type": "LCIA method data set", "refObjectId": "2299222a-bbd8-474f-9d4f-4dd1f18aea7c", "uri": "../lciamethods/2299222a-bbd8-474f-9d4f-4dd1f18aea7c.xml"}, "other": {"anies": [{"name": "referenceToUnitGroupDataSet", "value": {"shortDescription": [{"value": "CTUh", "lang": "en"}], "type": "unit group data set", "refObjectId": "d4c9523e-2d7e-49fd-8469-998f547d3a70", "uri": "../unitgroups/d4c9523e-2d7e-49fd-8469-998f547d3a70.xml"}}, {"value": "1.34230767194982E-06", "module": "A1-A3"}, {"value": "1.30954857615438E-12", "module": "A4"}, {"value": "5.40789281089108E-12", "module": "A5"}, {"value": "4.83652844032569E-12", "module": "C1"}, {"value": "8.50356218282064E-13", "module": "C2"}, {"value": "0", "module": "C3"}, {"value": "0", "module": "C4"}, {"value": "-6.39893029962326E-08", "module": "D"}]}}, {"referenceToLCIAMethodDataSet": {"shortDescription": [{"value": "Comparative toxic unit for humans (noncarcinogenic) (HTP-nc)", "lang": "en"}, {"value": "Toxizitätsvergleichseinheit für Menschen (nicht krebserregend) (HTP-nc)", "lang": "de"}], "type": "LCIA method data set", "refObjectId": "3af763a5-b7a1-48c9-9cee-1f223481fcef", "uri": "../lciamethods/3af763a5-b7a1-48c9-9cee-1f223481fcef.xml"}, "other": {"anies": [{"name": "referenceToUnitGroupDataSet", "value": {"shortDescription": [{"value": "CTUh", "lang": "en"}], "type": "unit group data set", "refObjectId": "d4c9523e-2d7e-49fd-8469-998f547d3a70", "uri": "../unitgroups/d4c9523e-2d7e-49fd-8469-998f547d3a70.xml"}}, {"value": "1.46480501842129E-07", "module": "A1-A3"}, {"value": "6.98355592286831E-11", "module": "A4"}, {"value": "2.71255736333156E-10", "module": "A5"}, {"value": "2.47571985381409E-10", "module": "C1"}, {"value": "4.53477657329111E-11", "module": "C2"}, {"value": "0", "module": "C3"}, {"value": "0", "module": "C4"}, {"value": "-3.26338586720344E-08", "module": "D"}]}}, {"referenceToLCIAMethodDataSet": {"shortDescription": [{"value": "Soil quality index (SQP)", "lang": "en"}, {"value": "Bodenqualitätsindex (SQP)", "lang": "de"}], "type": "LCIA method data set", "refObjectId": "b2ad6890-c78d-11e6-9d9d-cec0c932ce01", "uri": "../lciamethods/b2ad6890-c78d-11e6-9d9d-cec0c932ce01.xml"}, "other": {"anies": [{"name": "referenceToUnitGroupDataSet", "value": {"shortDescription": [{"value": "SQP", "lang": "en"}], "type": "unit group data set", "refObjectId": "f130951c-e67f-4f7f-8dd4-665de3974e18", "uri": "../unitgroups/f130951c-e67f-4f7f-8dd4-665de3974e18.xml"}}, {"value": "34.30443402192", "module": "A1-A3"}, {"value": "0.037649289209859", "module": "A4"}, {"value": "0.132949864809222", "module": "A5"}, {"value": "0.126640099634696", "module": "C1"}, {"value": "0.0244475903960121", "module": "C2"}, {"value": "0", "module": "C3"}, {"value": "0", "module": "C4"}, {"value": "-7.25870143389946", "module": "D"}]}}]}, "otherAttributes": {"{http://www.indata.network/EPD/2019}epd-version": "1.2"}, "version": "1.1", "locations": "../ILCDLocations.xml"}