{"processInformation": {"dataSetInformation": {"UUID": "f0b20a40-b4cb-4c34-9f2e-145e3d9af024", "name": {"baseName": [{"value": "FOAMGLAS® S3", "lang": "en"}, {"value": "FOAMGLAS® S3", "lang": "de"}], "functionalUnitFlowProperties": [{"lang": "en"}]}, "classificationInformation": {"classification": [{"class": [{"value": "Dämmstoffe", "level": 0, "classId": "2"}, {"value": "Schaumglas", "level": 1, "classId": "2.6"}, {"value": "Platten", "level": 2, "classId": "2.6.01"}], "name": "OEKOBAU.DAT"}, {"class": [{"value": "02 Building products", "level": 0}, {"value": "Thermal insulation products", "level": 1}, {"value": "Mineral insulating materials", "level": 2}], "name": "IBUCategories"}]}, "generalComment": [{"value": "FOAMGLAS® S3 is an insulation product for buildings made of cellular glass. It is applied to the desired dimensions in the form of slabs, panels, or other specific elements. The FOAMGLAS® S3 is in general unfaced as a slab. In some cases, depending on the end-use, the slabs can be faced with bitumen on the top with a PE-foil (e.g. FOAMGLAS® READY, BOARDS) or a white mineral liner (FOAMGLAS® ROOFBLOCK, ROOF BOARDS). Also, on the bottom, the white mineral liner can be applied (cf. BOARDS). \n\nThe product is declared with a density of 130 kg/m³ (±10%) and is supplied in thicknesses of 40 mm to 200 mm. \n\n\nFor the placing on the market of the product FOAMGLAS® S3 in the European Union/European Free Trade Association (EU/EFTA) (with the exception of Switzerland) Construction Products Regulation (CPR) applies. The product declaration of performance (DOP) is taking into consideration EN 13167:2015 Thermal insulation products for buildings – Factory made cellular glass (CG) products – Specification but also EN14305:2013 Thermal insulation for building equipment and industrial installations - Factory made cellular glass (CG) products – Specification. \n\nIn addition to the common applications, especially for loadbearing constructions and perimeter insulation, the product also complies with the characteristics declared in European Technical Assessment (ETA) 20/0221:2020 Cellular glass boards as load bearing layer and thermal insulation outside the waterproofing and the CE-marking.  For the application and use the respective national provisions apply.", "lang": "en"}, {"value": "Schaumglasplatten höherer Rohdichte mit sehr hoher Druckfestigkeit", "lang": "de"}], "other": {"anies": [{"scenario": [{"description": [{"value": "Scenario 1", "lang": "en"}, {"value": "Szenario 1", "lang": "de"}], "name": "S1"}, {"description": [{"value": "Scenario 2", "lang": "en"}, {"value": "Szenario 2", "lang": "de"}], "name": "S2"}, {"description": [{"value": "Scenario 3", "lang": "en"}, {"value": "Szenario 3", "lang": "de"}], "name": "S3"}]}]}}, "quantitativeReference": {"referenceToReferenceFlow": [0]}, "time": {"referenceYear": 2021, "dataSetValidUntil": 2026, "other": {"anies": [{"name": "publicationDateOfEPD", "value": 1615766400000}]}}, "geography": {"locationOfOperationSupplyOrProduction": {"location": "RER"}}, "technology": {"technologyDescriptionAndIncludedProcesses": [{"value": "The product is made following the protocol of the company. All glass constituents (recycled glass, sand, sodium carbonate, feldspar, sodium sulfate, sodium nitrate, iron oxide, and FOAMGLAS®-scrap) are melted (at ca. 1250°C) in the furnace and drawn into the shape of a thin-walled tube to enable efficient grinding. Melted glass from the melter furnace is put in grinders to produce fine glass powder. In the grinding process, additives are added so that afterwards, glass foaming processes can be envisaged. In the foaming furnace, cellular glass blocks are made in moulds by heating (sintering towards ca 850°C) the glass powder after the grinding process. After the foaming process, the annealing process starts by moving the foamed blocks on the lehr where they cool according to a precisely determined curve. The cooled blocks are cut into rectangular blocks and if necessary, ground or cut to thinner sizes. The produced material is released, labelled, marked, and packed for commercialisation and various end-use applications (floor, roof, wall, façade and other construction elements). 1 Mixing and batching of the raw materials: Recycled glass, feldspar, sodium carbonate, iron oxide, manganese oxide, sodium sulphate, sodium nitrate. 2 The melting furnace has a constant temperature of 1250°C. 3 Molten glass is drawn out of the furnace. 4 Control room for monitoring the production. 5 The glass is drawn off and falls onto the conveyor band where it cools down before entering the ball mill. 6 Addition of \"carbon black\". 7 Ball mill grinds all ingredients into a fine powder before putting them into stainless steel moulds. 8 The filled moulds pass through a cellulating oven (foaming furnace) with a temperature of 850°C. This is where the material gains its unique cell structure. 9 Energy recovery of heat. 10 The FOAMGLAS® blocks pass through an annealing oven to allow carefully controlled cooling without thermal stress. 11 The blocks are cut to size and sorted by batch. Production waste is recycled. 12 FOAMGLAS® slabs are then packaged, labelled and palletized. 13 Finished FOAMGLAS® products are stored and prepared for transport. Quality assurance Quality is assured through internal and external monitoring. The product complies with the Declaration of Performance. It also bears the CEN Keymark. \nTechnical data: \nThe technical specifications of FOAMGLAS® S3 within the scope of this EPD and within the CE marking is according to EN 13167 and ETA. In addition to the EN13167 declared values the same for the ETA, declared values on the mechanical properties, for loadbearing & below ground applications. Performance data of the product in accordance with the declaration of performance with respect to its essential characteristics according to EN 13167.  \n\nVoluntary data: CEN KEYMARK certificate n°001-BK-516-001; ATG H539; KOMO-CTG100-9; SIA CH672-13; ACERMI 023/253; Natureplus n°Zt-PCE-0406-1101-101 \nDeclared unit: \nThe Declaration refers to the life cycle of 1kg FOAMGLAS® S3. The gross density of the product is 130 kg / m³ ± 10%", "lang": "en"}, {"value": "Technische Daten: \nWärmeleitfähigkeit 0,045 W/m²K \nDeklarierte Einheit: \n1 kg FOAMGLAS® S3", "lang": "de"}], "technologicalApplicability": [{"value": "FOAMGLAS® S3 products are used for roof, floors, loadbearing, perimeter or specific other insulation.", "lang": "en"}, {"value": "Dämmstoff für die gesamte Gebäudehülle. Das Hauptanwendungsgebiet ist die Anwendung als Kompaktdach für langlebige Flachdachkonstruktionen.", "lang": "de"}]}}, "modellingAndValidation": {"LCIMethodAndAllocation": {"typeOfDataSet": "EPD", "referenceToLCAMethodDetails": [{"shortDescription": [{"value": "Mineral insulating materials.pdf", "lang": "en"}], "type": "source data set", "refObjectId": "728fa4ca-8499-4c28-8425-05af89b6ac19"}], "other": {"anies": [{"name": "subType", "value": "specific dataset"}]}}, "dataSourcesTreatmentAndRepresentativeness": {"referenceToDataSource": [{"shortDescription": [{"value": "GaBi Database (all versions)", "lang": "en"}], "type": "source data set", "refObjectId": "28d74cc0-db8b-4d7e-bc44-5f6d56ce0c4a"}, {"shortDescription": [{"value": "GaBi database SP40 2020", "lang": "en"}], "type": "source data set", "refObjectId": "0115289e-52f0-4920-bc7e-57b1c96aec8d"}], "useAdviceForDataSet": [{"value": "Scope: \nThis document refers to the production of 1 kg uncoated \"FOAMGLAS® S3\" cellular glass manufactured in Belgium at the Tessenderlo\n\nproduction facility of Pittsburgh Corning Europe NV. The reference year of production is 2019. The environmental impacts of the coated product \"FOAMGLAS® S3 in boards & blocks\" are to be assessed with the help of a markup factor in the amount of 0.8% for Global Warming Potential. \nSystem boundary: \nType of EPD: Cradle to Grave with options, modules C1-C4, and module D (A1-A3, C, D and additional modules)\n\nThe LCA addresses the life cycle stage of production, installation, end-of-life (EoL) and potential benefits beyond the system boundaries.\n\nThe product stage comprises of modules A1 (raw material supply), A2 (transport) and A3 (production). The following individual processes were included in the product stage A1- A3 of production:\n\nProcesses for providing preliminary products and energy\nTransporting the raw materials and preliminary materials to the plant\nThe manufacturing process in the plant including energy-related expenses, disposal of residual materials and emissions\nProduction of packaging\n\n\nModule A4 takes into account the transportation of product to the construction site. The treatment of the packaging materials is assigned to module A5 . Module C1 takes into accounts the de-construction or demolition of the product before taking it for treatment/disposal through means of transportation (module C2). Module C3 is the waste processing of the product before recycling/recovery/reuse. Landfilling with residual materials is assigned to module C4 . Module D accounts for the potential credits resulting from the thermal and electrical energy generated when burning packaging materials in module A5 (energy substitution).\n\nThere are 3 EoL scenarios in the study: Landfill, Reuse and Recycling. Module D/2 takes into account potential credits for 100% reuse of material and module D/3 considers potential credits for replacing kaolin in the brick industry.", "lang": "en"}, {"value": "Gültigkeitsbereich: \nDieses Dokument bezieht sich auf die Herstellung von\n1 kg unbeschichtetes Schaumglas „FOAMGLAS®\nS3“ hergestellt in Belgien am Produktionsstandort\nTessenderlo der Firma Pittsburgh Corning Europe NV sowie in Klasterec Tschechische Republik. \nSystemgrenze: \nTyp der EPD: Wiege-bis-Werkstor\nDie berechnete Ökobilanz adressiert das Lebenszyklusstadium\nder Produktherstellung. Aufwendungen für das Umschmelzen von End-of-Life\nSchrotten sowie Gutschriften für die im System\nanfallende Nettoschrottmenge und Gutschriften aus\nder thermischen Verwertung von Reststoffen sind dem\nModul D zugeordnet.", "lang": "de"}], "other": {"anies": [{"name": "referenceToOriginalEPD", "value": {"shortDescription": {"value": "FOAMGLAS® S3.pdf", "defaultValue": "FOAMGLAS® S3.pdf", "lstrings": [{"lang": "en", "value": "FOAMGLAS® S3.pdf"}]}, "type": "source data set", "uuid": {"uuid": "812c7e5b-31e6-4aba-8ca4-ec18bd3c1b9f"}, "refObjectId": "812c7e5b-31e6-4aba-8ca4-ec18bd3c1b9f", "resourceURLs": ["https://oekobaudat.de/OEKOBAU.DAT/resource/sources/812c7e5b-31e6-4aba-8ca4-ec18bd3c1b9f/FOAMGLAS_S3_12966.pdf?version=00.01.000"]}}]}}, "validation": {"review": [{"referenceToNameOfReviewerAndInstitution": [{"shortDescription": [{"value": "Institut Bauen und Umwelt e. V.", "lang": "en"}], "type": "contact data set", "refObjectId": "d111dbec-b024-4be5-86c5-752d6eb2cf95", "uri": "../contacts/d111dbec-b024-4be5-86c5-752d6eb2cf95.xml"}], "type": "Accredited third party review"}]}, "complianceDeclarations": {"compliance": [{"referenceToComplianceSystem": {"shortDescription": [{"value": "DIN EN 15804+A2", "lang": "en"}], "type": "source data set", "refObjectId": "c0016b33-8cf7-415c-ac6e-deba0d21440d", "uri": "../sources/c0016b33-8cf7-415c-ac6e-deba0d21440d.xml"}}, {"referenceToComplianceSystem": {"shortDescription": [{"value": "ISO 14025", "lang": "en"}], "type": "source data set", "refObjectId": "4f2eb655-6e44-4874-a95a-e28f5442cd4d", "uri": "../sources/4f2eb655-6e44-4874-a95a-e28f5442cd4d.xml"}}]}}, "administrativeInformation": {"commissionerAndGoal": {"referenceToCommissioner": [{"shortDescription": [{"value": "Pittsburgh Corning Europe NV", "lang": "en"}], "type": "contact data set", "refObjectId": "7decf5ec-2592-44cc-b676-fa81bb05cf72", "uri": "../contacts/7decf5ec-2592-44cc-b676-fa81bb05cf72.xml"}]}, "dataGenerator": {"referenceToPersonOrEntityGeneratingTheDataSet": [{"shortDescription": [{"value": "Sphera Solutions GmbH", "lang": "en"}], "type": "contact data set", "refObjectId": "623edf96-39d1-4e6f-9892-674c7228546b", "uri": "../contacts/623edf96-39d1-4e6f-9892-674c7228546b.xml"}]}, "dataEntryBy": {"timeStamp": 1615832302725, "referenceToDataSetFormat": [{"shortDescription": [{"value": "ILCD Format", "lang": "en"}], "type": "source data set", "refObjectId": "a97a0155-0234-4b87-b4ce-a45da52f2a40", "uri": "../sources/a97a0155-0234-4b87-b4ce-a45da52f2a40.xml"}, {"shortDescription": [{"value": "EPD-Datenformaterweiterungen v1.2", "lang": "de"}, {"value": "EPD Data Format Extensions v1.2", "lang": "en"}], "type": "source data set", "refObjectId": "a29449fd-aa2f-4de8-b5d7-4b06b43c6fde", "uri": "../sources/a29449fd-aa2f-4de8-b5d7-4b06b43c6fde.xml"}]}, "publicationAndOwnership": {"dataSetVersion": "00.03.000", "referenceToPrecedingDataSetVersion": [{"shortDescription": [{"value": "FOAMGLAS® S3", "lang": "en"}], "type": "process data set", "refObjectId": "9ca6d998-da4f-42f7-a2dc-565a89134cce", "uri": "../processes/9ca6d998-da4f-42f7-a2dc-565a89134cce.xml"}], "referenceToRegistrationAuthority": {"shortDescription": [{"value": "Institut Bauen und Umwelt e. V.", "lang": "en"}], "type": "contact data set", "refObjectId": "d111dbec-b024-4be5-86c5-752d6eb2cf95", "uri": "../contacts/d111dbec-b024-4be5-86c5-752d6eb2cf95.xml"}, "registrationNumber": "EPD-PCE-20200302-IBA1-EN", "referenceToOwnershipOfDataSet": {"shortDescription": [{"value": "Pittsburgh Corning Europe NV", "lang": "en"}], "type": "contact data set", "refObjectId": "7decf5ec-2592-44cc-b676-fa81bb05cf72", "uri": "../contacts/7decf5ec-2592-44cc-b676-fa81bb05cf72.xml"}, "copyright": true, "licenseType": "Free of charge for all users and uses", "accessRestrictions": [{"value": "None", "lang": "en"}], "other": {"anies": [{"name": "referenceToPublisher", "value": {"shortDescription": [{"value": "Institut Bauen und Umwelt e. V.", "lang": "en"}], "type": "contact data set", "refObjectId": "d111dbec-b024-4be5-86c5-752d6eb2cf95", "uri": "../contacts/d111dbec-b024-4be5-86c5-752d6eb2cf95.xml"}}]}}}, "exchanges": {"exchange": [{"dataSetInternalID": 0, "referenceToFlowDataSet": {"shortDescription": [{"value": "FOAMGLAS® S3 (1 kg FOAMGLAS® S3)", "lang": "en"}], "type": "flow data set", "refObjectId": "6014b18f-afdf-51da-7836-f2816b5822a8", "uri": "../flows/6014b18f-afdf-51da-7836-f2816b5822a8.xml"}, "meanAmount": 1.0, "referencesToDataSource": {}, "referenceFlow": true, "resolvedFlowVersion": "00.04.000", "resultingflowAmount": 1.0, "flowProperties": [{"name": [{"lang": "en", "value": "Mass"}, {"lang": "de", "value": "Masse"}], "uuid": "93a60a56-a3c8-11da-a746-0800200b9a66", "referenceFlowProperty": true, "meanValue": 1.0, "referenceUnit": "kg", "unitGroupUUID": "ad38d542-3fe9-439d-9b95-2f5f7752acaf"}], "materialProperties": [{"name": "gross density", "value": "130.0", "unit": "kg/m^3", "unitDescription": "kilograms per cubic metre"}], "typeOfFlow": "Product flow", "classification": {"classHierarchy": "Dämmstoffe / Schaumglas / Foamglas", "name": "OEKOBAU.DAT"}}, {"dataSetInternalID": 1, "referenceToFlowDataSet": {"shortDescription": [{"value": "Renewable primary energy as energy carrier (PERE)", "lang": "en"}, {"value": "Erneuerbare Primärenergie als Energieträger (PERE)", "lang": "de"}], "type": "flow data set", "refObjectId": "20f32be5-0398-4288-9b6d-accddd195317", "uri": "../flows/20f32be5-0398-4288-9b6d-accddd195317.xml"}, "exchange direction": "INPUT", "other": {"anies": [{"name": "referenceToUnitGroupDataSet", "value": {"shortDescription": [{"value": "MJ", "lang": "en"}], "type": "unit group data set", "refObjectId": "93a60a57-a3c8-11da-a746-0800200c9a66", "uri": "../unitgroups/93a60a57-a3c8-11da-a746-0800200c9a66.xml"}}, {"value": "12.5", "module": "A1-A3"}, {"value": "0.0211", "module": "A4"}, {"value": "0.808", "module": "A5"}, {"value": "0.000461", "module": "C1"}, {"value": "0.00167", "module": "C2"}, {"value": "0", "module": "C3", "scenario": "S2"}, {"value": "0.0211", "module": "C3", "scenario": "S3"}, {"value": "0.0261", "module": "C4"}, {"value": "-0.168", "module": "D", "scenario": "S0"}, {"value": "-12.5", "module": "D", "scenario": "S2"}, {"value": "-0.134", "module": "D", "scenario": "S3"}]}, "resolvedFlowVersion": "38.00.000", "flowProperties": [], "typeOfFlow": "Other flow", "classification": {"classHierarchy": "Quantities", "name": "GaBiCategories"}}, {"dataSetInternalID": 2, "referenceToFlowDataSet": {"shortDescription": [{"value": "Renewable primary energy resources as material utilization (PERM)", "lang": "en"}, {"value": "Erneuerbare Primärenergie zur stofflichen Nutzung (PERM)", "lang": "de"}], "type": "flow data set", "refObjectId": "fb3ec0de-548d-4508-aea5-00b73bf6f702", "uri": "../flows/fb3ec0de-548d-4508-aea5-00b73bf6f702.xml"}, "exchange direction": "INPUT", "other": {"anies": [{"name": "referenceToUnitGroupDataSet", "value": {"shortDescription": [{"value": "MJ", "lang": "en"}], "type": "unit group data set", "refObjectId": "93a60a57-a3c8-11da-a746-0800200c9a66", "uri": "../unitgroups/93a60a57-a3c8-11da-a746-0800200c9a66.xml"}}, {"value": "0.8", "module": "A1-A3"}, {"value": "0", "module": "A4"}, {"value": "-0.8", "module": "A5"}, {"value": "0", "module": "C1"}, {"value": "0", "module": "C2"}, {"value": "0", "module": "C3", "scenario": "S2"}, {"value": "0", "module": "C3", "scenario": "S3"}, {"value": "0", "module": "C4"}, {"value": "0", "module": "D", "scenario": "S0"}, {"value": "-0.8", "module": "D", "scenario": "S2"}, {"value": "0", "module": "D", "scenario": "S3"}]}, "resolvedFlowVersion": "38.00.000", "flowProperties": [], "typeOfFlow": "Other flow", "classification": {"classHierarchy": "Quantities", "name": "GaBiCategories"}}, {"dataSetInternalID": 3, "referenceToFlowDataSet": {"shortDescription": [{"value": "Total use of renewable primary energy resources (PERT)", "lang": "en"}, {"value": "Total erneuerbare Primärenergie (PERT)", "lang": "de"}], "type": "flow data set", "refObjectId": "53f97275-fa8a-4cdd-9024-65936002acd0", "uri": "../flows/53f97275-fa8a-4cdd-9024-65936002acd0.xml"}, "exchange direction": "INPUT", "other": {"anies": [{"name": "referenceToUnitGroupDataSet", "value": {"shortDescription": [{"value": "MJ", "lang": "en"}], "type": "unit group data set", "refObjectId": "93a60a57-a3c8-11da-a746-0800200c9a66", "uri": "../unitgroups/93a60a57-a3c8-11da-a746-0800200c9a66.xml"}}, {"value": "13.3", "module": "A1-A3"}, {"value": "0.0211", "module": "A4"}, {"value": "0.00800000000000001", "module": "A5"}, {"value": "0.000461", "module": "C1"}, {"value": "0.00167", "module": "C2"}, {"value": "0", "module": "C3", "scenario": "S2"}, {"value": "0.0211", "module": "C3", "scenario": "S3"}, {"value": "0.0261", "module": "C4"}, {"value": "-0.168", "module": "D", "scenario": "S0"}, {"value": "-13.3", "module": "D", "scenario": "S2"}, {"value": "-0.134", "module": "D", "scenario": "S3"}]}, "resolvedFlowVersion": "38.00.000", "flowProperties": [], "typeOfFlow": "Other flow", "classification": {"classHierarchy": "Quantities / Environmental quantities / EPD EN 15804 / LCI indicators", "name": "GaBiCategories"}}, {"dataSetInternalID": 4, "referenceToFlowDataSet": {"shortDescription": [{"value": "Non renewable primary energy as energy carrier (PENRE)", "lang": "en"}, {"value": "Nicht-erneuerbare Primärenergie als Energieträger (PENRE)", "lang": "de"}], "type": "flow data set", "refObjectId": "ac857178-2b45-46ec-892a-a9a4332f0372", "uri": "../flows/ac857178-2b45-46ec-892a-a9a4332f0372.xml"}, "exchange direction": "INPUT", "other": {"anies": [{"name": "referenceToUnitGroupDataSet", "value": {"shortDescription": [{"value": "MJ", "lang": "en"}], "type": "unit group data set", "refObjectId": "93a60a57-a3c8-11da-a746-0800200c9a66", "uri": "../unitgroups/93a60a57-a3c8-11da-a746-0800200c9a66.xml"}}, {"value": "21.3", "module": "A1-A3"}, {"value": "0.376", "module": "A4"}, {"value": "0.566", "module": "A5"}, {"value": "0.00821", "module": "C1"}, {"value": "0.0298", "module": "C2"}, {"value": "0", "module": "C3", "scenario": "S2"}, {"value": "0.0476", "module": "C3", "scenario": "S3"}, {"value": "0.199", "module": "C4"}, {"value": "-0.804", "module": "D", "scenario": "S0"}, {"value": "-21.3", "module": "D", "scenario": "S2"}, {"value": "-3.29", "module": "D", "scenario": "S3"}]}, "resolvedFlowVersion": "38.00.000", "flowProperties": [], "typeOfFlow": "Other flow", "classification": {"classHierarchy": "Quantities", "name": "GaBiCategories"}}, {"dataSetInternalID": 5, "referenceToFlowDataSet": {"shortDescription": [{"value": "Non renewable primary energy as material utilization (PENRM)", "lang": "en"}, {"value": "Nicht-erneuerbare Primärenergie zur stofflichen Nutzung (PENRM)", "lang": "de"}], "type": "flow data set", "refObjectId": "1421caa0-679d-4bf4-b282-0eb850ccae27", "uri": "../flows/1421caa0-679d-4bf4-b282-0eb850ccae27.xml"}, "exchange direction": "INPUT", "other": {"anies": [{"name": "referenceToUnitGroupDataSet", "value": {"shortDescription": [{"value": "MJ", "lang": "en"}], "type": "unit group data set", "refObjectId": "93a60a57-a3c8-11da-a746-0800200c9a66", "uri": "../unitgroups/93a60a57-a3c8-11da-a746-0800200c9a66.xml"}}, {"value": "0.53", "module": "A1-A3"}, {"value": "0", "module": "A4"}, {"value": "-0.53", "module": "A5"}, {"value": "0", "module": "C1"}, {"value": "0", "module": "C2"}, {"value": "0", "module": "C3", "scenario": "S2"}, {"value": "0", "module": "C3", "scenario": "S3"}, {"value": "0", "module": "C4"}, {"value": "0", "module": "D", "scenario": "S0"}, {"value": "-0.53", "module": "D", "scenario": "S2"}, {"value": "0", "module": "D", "scenario": "S3"}]}, "resolvedFlowVersion": "38.00.000", "flowProperties": [], "typeOfFlow": "Other flow", "classification": {"classHierarchy": "Quantities", "name": "GaBiCategories"}}, {"dataSetInternalID": 6, "referenceToFlowDataSet": {"shortDescription": [{"value": "Total use of non renewable primary energy resources (PENRT)", "lang": "en"}, {"value": "Total nicht erneuerbare Primärenergie (PENRT)", "lang": "de"}], "type": "flow data set", "refObjectId": "06159210-646b-4c8d-8583-da9b3b95a6c1", "uri": "../flows/06159210-646b-4c8d-8583-da9b3b95a6c1.xml"}, "exchange direction": "INPUT", "other": {"anies": [{"name": "referenceToUnitGroupDataSet", "value": {"shortDescription": [{"value": "MJ", "lang": "en"}], "type": "unit group data set", "refObjectId": "93a60a57-a3c8-11da-a746-0800200c9a66", "uri": "../unitgroups/93a60a57-a3c8-11da-a746-0800200c9a66.xml"}}, {"value": "21.83", "module": "A1-A3"}, {"value": "0.376", "module": "A4"}, {"value": "0.0359999999999999", "module": "A5"}, {"value": "0.00821", "module": "C1"}, {"value": "0.0298", "module": "C2"}, {"value": "0", "module": "C3", "scenario": "S2"}, {"value": "0.0476", "module": "C3", "scenario": "S3"}, {"value": "0.199", "module": "C4"}, {"value": "-0.804", "module": "D", "scenario": "S0"}, {"value": "-21.83", "module": "D", "scenario": "S2"}, {"value": "-3.29", "module": "D", "scenario": "S3"}]}, "resolvedFlowVersion": "38.00.000", "flowProperties": [], "typeOfFlow": "Other flow", "classification": {"classHierarchy": "Quantities / Environmental quantities / EPD EN 15804 / LCI indicators", "name": "GaBiCategories"}}, {"dataSetInternalID": 7, "referenceToFlowDataSet": {"shortDescription": [{"value": "Use of secondary material (SM)", "lang": "en"}, {"value": "Einsatz von Sekundärstoffen (SM)", "lang": "de"}], "type": "flow data set", "refObjectId": "c6a1f35f-2d09-4f54-8dfb-97e502e1ce92", "uri": "../flows/c6a1f35f-2d09-4f54-8dfb-97e502e1ce92.xml"}, "exchange direction": "INPUT", "other": {"anies": [{"name": "referenceToUnitGroupDataSet", "value": {"shortDescription": [{"value": "kg", "lang": "en"}], "type": "unit group data set", "refObjectId": "ad38d542-3fe9-439d-9b95-2f5f7752acaf", "uri": "../unitgroups/ad38d542-3fe9-439d-9b95-2f5f7752acaf.xml"}}, {"value": "0.383", "module": "A1-A3"}, {"value": "0", "module": "A4"}, {"value": "0", "module": "A5"}, {"value": "0", "module": "C1"}, {"value": "0", "module": "C2"}, {"value": "0", "module": "C3", "scenario": "S2"}, {"value": "0", "module": "C3", "scenario": "S3"}, {"value": "0", "module": "C4"}, {"value": "0", "module": "D", "scenario": "S0"}, {"value": "0", "module": "D", "scenario": "S2"}, {"value": "0", "module": "D", "scenario": "S3"}]}, "resolvedFlowVersion": "38.00.000", "flowProperties": [], "typeOfFlow": "Other flow", "classification": {"classHierarchy": "Quantities / Environmental quantities / EPD EN 15804 / LCI indicators", "name": "GaBiCategories"}}, {"dataSetInternalID": 8, "referenceToFlowDataSet": {"shortDescription": [{"value": "Use of renewable secondary fuels (RSF)", "lang": "en"}, {"value": "Erneuerbare Sekundärbrennstoffe (RSF)", "lang": "de"}], "type": "flow data set", "refObjectId": "64333088-a55f-4aa2-9a31-c10b07816787", "uri": "../flows/64333088-a55f-4aa2-9a31-c10b07816787.xml"}, "exchange direction": "INPUT", "other": {"anies": [{"name": "referenceToUnitGroupDataSet", "value": {"shortDescription": [{"value": "MJ", "lang": "en"}], "type": "unit group data set", "refObjectId": "93a60a57-a3c8-11da-a746-0800200c9a66", "uri": "../unitgroups/93a60a57-a3c8-11da-a746-0800200c9a66.xml"}}, {"value": "0", "module": "A1-A3"}, {"value": "0", "module": "A4"}, {"value": "0", "module": "A5"}, {"value": "0", "module": "C1"}, {"value": "0", "module": "C2"}, {"value": "0", "module": "C3", "scenario": "S2"}, {"value": "0", "module": "C3", "scenario": "S3"}, {"value": "0", "module": "C4"}, {"value": "0", "module": "D", "scenario": "S0"}, {"value": "0", "module": "D", "scenario": "S2"}, {"value": "0", "module": "D", "scenario": "S3"}]}, "resolvedFlowVersion": "38.00.000", "flowProperties": [], "typeOfFlow": "Other flow", "classification": {"classHierarchy": "Quantities / Environmental quantities / EPD EN 15804 / LCI indicators", "name": "GaBiCategories"}}, {"dataSetInternalID": 9, "referenceToFlowDataSet": {"shortDescription": [{"value": "Use of non renewable secondary fuels (NRSF)", "lang": "en"}, {"value": "Nicht erneuerbare Sekundärbrennstoffe (NRSF)", "lang": "de"}], "type": "flow data set", "refObjectId": "89def144-d39a-4287-b86f-efde453ddcb2", "uri": "../flows/89def144-d39a-4287-b86f-efde453ddcb2.xml"}, "exchange direction": "INPUT", "other": {"anies": [{"name": "referenceToUnitGroupDataSet", "value": {"shortDescription": [{"value": "MJ", "lang": "en"}], "type": "unit group data set", "refObjectId": "93a60a57-a3c8-11da-a746-0800200c9a66", "uri": "../unitgroups/93a60a57-a3c8-11da-a746-0800200c9a66.xml"}}, {"value": "0", "module": "A1-A3"}, {"value": "0", "module": "A4"}, {"value": "0", "module": "A5"}, {"value": "0", "module": "C1"}, {"value": "0", "module": "C2"}, {"value": "0", "module": "C3", "scenario": "S2"}, {"value": "0", "module": "C3", "scenario": "S3"}, {"value": "0", "module": "C4"}, {"value": "0", "module": "D", "scenario": "S0"}, {"value": "0", "module": "D", "scenario": "S2"}, {"value": "0", "module": "D", "scenario": "S3"}]}, "resolvedFlowVersion": "38.00.000", "flowProperties": [], "typeOfFlow": "Other flow", "classification": {"classHierarchy": "Quantities / Environmental quantities / EPD EN 15804 / LCI indicators", "name": "GaBiCategories"}}, {"dataSetInternalID": 10, "referenceToFlowDataSet": {"shortDescription": [{"value": "Use of net fresh water (FW)", "lang": "en"}, {"value": "Einsatz von Süßwasserressourcen (FW)", "lang": "de"}], "type": "flow data set", "refObjectId": "3cf952c8-f3a4-461d-8c96-96456ca62246", "uri": "../flows/3cf952c8-f3a4-461d-8c96-96456ca62246.xml"}, "exchange direction": "INPUT", "other": {"anies": [{"name": "referenceToUnitGroupDataSet", "value": {"shortDescription": [{"value": "m^3", "lang": "en"}], "type": "unit group data set", "refObjectId": "cd950537-0a98-4044-9ba7-9f9a68d0a504", "uri": "../unitgroups/cd950537-0a98-4044-9ba7-9f9a68d0a504.xml"}}, {"value": "0.0259", "module": "A1-A3"}, {"value": "2.44E-05", "module": "A4"}, {"value": "0.000305", "module": "A5"}, {"value": "5.34E-07", "module": "C1"}, {"value": "1.94E-06", "module": "C2"}, {"value": "0", "module": "C3", "scenario": "S2"}, {"value": "2.44E-05", "module": "C3", "scenario": "S3"}, {"value": "5.02E-05", "module": "C4"}, {"value": "-0.000195", "module": "D", "scenario": "S0"}, {"value": "-0.0259", "module": "D", "scenario": "S2"}, {"value": "-0.000157", "module": "D", "scenario": "S3"}]}, "resolvedFlowVersion": "38.00.000", "flowProperties": [], "typeOfFlow": "Other flow", "classification": {"classHierarchy": "Quantities / Environmental quantities / EPD EN 15804 / LCI indicators", "name": "GaBiCategories"}}, {"dataSetInternalID": 11, "referenceToFlowDataSet": {"shortDescription": [{"value": "Hazardous waste disposed (HWD)", "lang": "en"}, {"value": "Gefährlicher Abfall zur Deponie (HWD)", "lang": "de"}], "type": "flow data set", "refObjectId": "430f9e0f-59b2-46a0-8e0d-55e0e84948fc", "uri": "../flows/430f9e0f-59b2-46a0-8e0d-55e0e84948fc.xml"}, "exchange direction": "OUTPUT", "other": {"anies": [{"name": "referenceToUnitGroupDataSet", "value": {"shortDescription": [{"value": "kg", "lang": "en"}], "type": "unit group data set", "refObjectId": "ad38d542-3fe9-439d-9b95-2f5f7752acaf", "uri": "../unitgroups/ad38d542-3fe9-439d-9b95-2f5f7752acaf.xml"}}, {"value": "6.77E-08", "module": "A1-A3"}, {"value": "1.75E-08", "module": "A4"}, {"value": "7.55E-11", "module": "A5"}, {"value": "3.82E-10", "module": "C1"}, {"value": "1.39E-09", "module": "C2"}, {"value": "0", "module": "C3", "scenario": "S2"}, {"value": "1.97E-11", "module": "C3", "scenario": "S3"}, {"value": "3.03E-09", "module": "C4"}, {"value": "-3.2E-10", "module": "D", "scenario": "S0"}, {"value": "-6.77E-08", "module": "D", "scenario": "S2"}, {"value": "-2.77E-09", "module": "D", "scenario": "S3"}]}, "resolvedFlowVersion": "38.00.000", "flowProperties": [], "typeOfFlow": "Other flow", "classification": {"classHierarchy": "Quantities / Environmental quantities / EPD EN 15804 / LCI indicators", "name": "GaBiCategories"}}, {"dataSetInternalID": 12, "referenceToFlowDataSet": {"shortDescription": [{"value": "Non hazardous waste disposed (NHWD)", "lang": "en"}, {"value": "Entsorgter nicht gefährlicher Abfall (NHWD)", "lang": "de"}], "type": "flow data set", "refObjectId": "b29ef66b-e286-4afa-949f-62f1a7b4d7fa", "uri": "../flows/b29ef66b-e286-4afa-949f-62f1a7b4d7fa.xml"}, "exchange direction": "OUTPUT", "other": {"anies": [{"name": "referenceToUnitGroupDataSet", "value": {"shortDescription": [{"value": "kg", "lang": "en"}], "type": "unit group data set", "refObjectId": "ad38d542-3fe9-439d-9b95-2f5f7752acaf", "uri": "../unitgroups/ad38d542-3fe9-439d-9b95-2f5f7752acaf.xml"}}, {"value": "0.0406", "module": "A1-A3"}, {"value": "5.75E-05", "module": "A4"}, {"value": "0.00434", "module": "A5"}, {"value": "1.26E-06", "module": "C1"}, {"value": "4.56E-06", "module": "C2"}, {"value": "0", "module": "C3", "scenario": "S2"}, {"value": "3.37E-05", "module": "C3", "scenario": "S3"}, {"value": "1", "module": "C4"}, {"value": "-0.000363", "module": "D", "scenario": "S0"}, {"value": "-0.0406", "module": "D", "scenario": "S2"}, {"value": "-0.000873", "module": "D", "scenario": "S3"}]}, "resolvedFlowVersion": "38.00.000", "flowProperties": [], "typeOfFlow": "Other flow", "classification": {"classHierarchy": "Quantities / Environmental quantities / EPD EN 15804 / LCI indicators", "name": "GaBiCategories"}}, {"dataSetInternalID": 13, "referenceToFlowDataSet": {"shortDescription": [{"value": "Radioactive waste disposed (RWD)", "lang": "en"}, {"value": "Entsorgter radioaktiver Abfall (RWD)", "lang": "de"}], "type": "flow data set", "refObjectId": "3449546e-52ad-4b39-b809-9fb77cea8ff6", "uri": "../flows/3449546e-52ad-4b39-b809-9fb77cea8ff6.xml"}, "exchange direction": "OUTPUT", "other": {"anies": [{"name": "referenceToUnitGroupDataSet", "value": {"shortDescription": [{"value": "kg", "lang": "en"}], "type": "unit group data set", "refObjectId": "ad38d542-3fe9-439d-9b95-2f5f7752acaf", "uri": "../unitgroups/ad38d542-3fe9-439d-9b95-2f5f7752acaf.xml"}}, {"value": "9.46E-05", "module": "A1-A3"}, {"value": "4.65E-07", "module": "A4"}, {"value": "1.72E-06", "module": "A5"}, {"value": "1.02E-08", "module": "C1"}, {"value": "3.68E-08", "module": "C2"}, {"value": "0", "module": "C3", "scenario": "S2"}, {"value": "7.22E-06", "module": "C3", "scenario": "S3"}, {"value": "2.26E-06", "module": "C4"}, {"value": "-5.75E-05", "module": "D", "scenario": "S0"}, {"value": "-9.46E-05", "module": "D", "scenario": "S2"}, {"value": "-4.4E-05", "module": "D", "scenario": "S3"}]}, "resolvedFlowVersion": "38.00.000", "flowProperties": [], "typeOfFlow": "Other flow", "classification": {"classHierarchy": "Quantities / Environmental quantities / EPD EN 15804 / LCI indicators", "name": "GaBiCategories"}}, {"dataSetInternalID": 14, "referenceToFlowDataSet": {"shortDescription": [{"value": "Components for re-use (CRU)", "lang": "en"}, {"value": "Komponenten für die Wiederverwendung (CRU)", "lang": "de"}], "type": "flow data set", "refObjectId": "a2b32f97-3fc7-4af2-b209-525bc6426f33", "uri": "../flows/a2b32f97-3fc7-4af2-b209-525bc6426f33.xml"}, "exchange direction": "OUTPUT", "other": {"anies": [{"name": "referenceToUnitGroupDataSet", "value": {"shortDescription": [{"value": "kg", "lang": "en"}], "type": "unit group data set", "refObjectId": "ad38d542-3fe9-439d-9b95-2f5f7752acaf", "uri": "../unitgroups/ad38d542-3fe9-439d-9b95-2f5f7752acaf.xml"}}, {"value": "0", "module": "A1-A3"}, {"value": "0", "module": "A4"}, {"value": "0", "module": "A5"}, {"value": "0", "module": "C1"}, {"value": "0", "module": "C2"}, {"value": "1", "module": "C3", "scenario": "S2"}, {"value": "0", "module": "C3", "scenario": "S3"}, {"value": "0", "module": "C4"}, {"value": "0", "module": "D", "scenario": "S0"}, {"value": "0", "module": "D", "scenario": "S2"}, {"value": "0", "module": "D", "scenario": "S3"}]}, "resolvedFlowVersion": "38.00.000", "flowProperties": [], "typeOfFlow": "Other flow", "classification": {"classHierarchy": "Quantities / Environmental quantities / EPD EN 15804 / LCI indicators", "name": "GaBiCategories"}}, {"dataSetInternalID": 15, "referenceToFlowDataSet": {"shortDescription": [{"value": "Materials for recycling (MFR)", "lang": "en"}, {"value": "Stoffe zum Recycling (MFR)", "lang": "de"}], "type": "flow data set", "refObjectId": "d7fe48a5-4103-49c8-9aae-b0b5dfdbd6ae", "uri": "../flows/d7fe48a5-4103-49c8-9aae-b0b5dfdbd6ae.xml"}, "exchange direction": "OUTPUT", "other": {"anies": [{"name": "referenceToUnitGroupDataSet", "value": {"shortDescription": [{"value": "kg", "lang": "en"}], "type": "unit group data set", "refObjectId": "ad38d542-3fe9-439d-9b95-2f5f7752acaf", "uri": "../unitgroups/ad38d542-3fe9-439d-9b95-2f5f7752acaf.xml"}}, {"value": "0", "module": "A1-A3"}, {"value": "0", "module": "A4"}, {"value": "0", "module": "A5"}, {"value": "0", "module": "C1"}, {"value": "0", "module": "C2"}, {"value": "0", "module": "C3", "scenario": "S2"}, {"value": "0.617", "module": "C3", "scenario": "S3"}, {"value": "0", "module": "C4"}, {"value": "0", "module": "D", "scenario": "S0"}, {"value": "0", "module": "D", "scenario": "S2"}, {"value": "0", "module": "D", "scenario": "S3"}]}, "resolvedFlowVersion": "38.00.000", "flowProperties": [], "typeOfFlow": "Other flow", "classification": {"classHierarchy": "Quantities / Environmental quantities / EPD EN 15804 / LCI indicators", "name": "GaBiCategories"}}, {"dataSetInternalID": 16, "referenceToFlowDataSet": {"shortDescription": [{"value": "Materials for energy recovery (MER)", "lang": "en"}, {"value": "Stoffe für die Energierückgewinnung (MER)", "lang": "de"}], "type": "flow data set", "refObjectId": "59a9181c-3aaf-46ee-8b13-2b3723b6e447", "uri": "../flows/59a9181c-3aaf-46ee-8b13-2b3723b6e447.xml"}, "exchange direction": "OUTPUT", "other": {"anies": [{"name": "referenceToUnitGroupDataSet", "value": {"shortDescription": [{"value": "kg", "lang": "en"}], "type": "unit group data set", "refObjectId": "ad38d542-3fe9-439d-9b95-2f5f7752acaf", "uri": "../unitgroups/ad38d542-3fe9-439d-9b95-2f5f7752acaf.xml"}}, {"value": "0", "module": "A1-A3"}, {"value": "0", "module": "A4"}, {"value": "0.0642", "module": "A5"}, {"value": "0", "module": "C1"}, {"value": "0", "module": "C2"}, {"value": "0", "module": "C3", "scenario": "S2"}, {"value": "0", "module": "C3", "scenario": "S3"}, {"value": "0", "module": "C4"}, {"value": "0", "module": "D", "scenario": "S0"}, {"value": "0", "module": "D", "scenario": "S2"}, {"value": "0", "module": "D", "scenario": "S3"}]}, "resolvedFlowVersion": "38.00.000", "flowProperties": [], "typeOfFlow": "Other flow", "classification": {"classHierarchy": "Quantities / Environmental quantities / EPD EN 15804 / LCI indicators", "name": "GaBiCategories"}}, {"dataSetInternalID": 17, "referenceToFlowDataSet": {"shortDescription": [{"value": "Exported electrical energy (EEE)", "lang": "en"}, {"value": "Exportierte elektrische Energie (EEE)", "lang": "de"}], "type": "flow data set", "refObjectId": "4da0c987-2b76-40d6-9e9e-82a017aaaf29", "uri": "../flows/4da0c987-2b76-40d6-9e9e-82a017aaaf29.xml"}, "exchange direction": "OUTPUT", "other": {"anies": [{"name": "referenceToUnitGroupDataSet", "value": {"shortDescription": [{"value": "MJ", "lang": "en"}], "type": "unit group data set", "refObjectId": "93a60a57-a3c8-11da-a746-0800200c9a66", "uri": "../unitgroups/93a60a57-a3c8-11da-a746-0800200c9a66.xml"}}, {"value": "0", "module": "A1-A3"}, {"value": "0", "module": "A4"}, {"value": "0.192", "module": "A5"}, {"value": "0", "module": "C1"}, {"value": "0", "module": "C2"}, {"value": "0", "module": "C3", "scenario": "S2"}, {"value": "0", "module": "C3", "scenario": "S3"}, {"value": "0", "module": "C4"}, {"value": "0", "module": "D", "scenario": "S0"}, {"value": "0", "module": "D", "scenario": "S2"}, {"value": "0", "module": "D", "scenario": "S3"}]}, "resolvedFlowVersion": "38.00.000", "flowProperties": [], "typeOfFlow": "Other flow", "classification": {"classHierarchy": "Quantities / Environmental quantities / EPD EN 15804 / LCI indicators", "name": "GaBiCategories"}}, {"dataSetInternalID": 18, "referenceToFlowDataSet": {"shortDescription": [{"value": "Exported thermal energy (EET)", "lang": "en"}, {"value": "Exportierte thermische Energie (EET)", "lang": "de"}], "type": "flow data set", "refObjectId": "98daf38a-7a79-46d3-9a37-2b7bd0955810", "uri": "../flows/98daf38a-7a79-46d3-9a37-2b7bd0955810.xml"}, "exchange direction": "OUTPUT", "other": {"anies": [{"name": "referenceToUnitGroupDataSet", "value": {"shortDescription": [{"value": "MJ", "lang": "en"}], "type": "unit group data set", "refObjectId": "93a60a57-a3c8-11da-a746-0800200c9a66", "uri": "../unitgroups/93a60a57-a3c8-11da-a746-0800200c9a66.xml"}}, {"value": "0", "module": "A1-A3"}, {"value": "0", "module": "A4"}, {"value": "0.377", "module": "A5"}, {"value": "0", "module": "C1"}, {"value": "0", "module": "C2"}, {"value": "0", "module": "C3", "scenario": "S2"}, {"value": "0", "module": "C3", "scenario": "S3"}, {"value": "0", "module": "C4"}, {"value": "0", "module": "D", "scenario": "S0"}, {"value": "0", "module": "D", "scenario": "S2"}, {"value": "0", "module": "D", "scenario": "S3"}]}, "resolvedFlowVersion": "38.00.000", "flowProperties": [], "typeOfFlow": "Other flow", "classification": {"classHierarchy": "Quantities / Environmental quantities / EPD EN 15804 / LCI indicators", "name": "GaBiCategories"}}]}, "LCIAResults": {"LCIAResult": [{"referenceToLCIAMethodDataSet": {"shortDescription": [{"value": "Global Warming Potential total (GWP-total)", "lang": "en"}, {"value": "Globales Erwärmungspotenzial total (GWP-total)", "lang": "de"}], "type": "LCIA method data set", "refObjectId": "6a37f984-a4b3-458a-a20a-64418c145fa2", "uri": "../lciamethods/6a37f984-a4b3-458a-a20a-64418c145fa2.xml"}, "other": {"anies": [{"name": "referenceToUnitGroupDataSet", "value": {"shortDescription": [{"value": "kg CO_(2)-Äq.", "lang": "en"}], "type": "unit group data set", "refObjectId": "1ebf3012-d0db-4de2-aefd-ef30cedb0be1", "uri": "../unitgroups/1ebf3012-d0db-4de2-aefd-ef30cedb0be1.xml"}}, {"value": "1.438", "module": "A1-A3"}, {"value": "0.0297", "module": "A4"}, {"value": "0.1236", "module": "A5"}, {"value": "0.00065", "module": "C1"}, {"value": "0.00236", "module": "C2"}, {"value": "0", "module": "C3", "scenario": "S2"}, {"value": "0.00274", "module": "C3", "scenario": "S3"}, {"value": "0.0153", "module": "C4"}, {"value": "-0.0475", "module": "D", "scenario": "S0"}, {"value": "-1.438", "module": "D", "scenario": "S2"}, {"value": "-0.2004", "module": "D", "scenario": "S3"}]}}, {"referenceToLCIAMethodDataSet": {"shortDescription": [{"value": "Global Warming Potential fossil fuels (GWP-fossil)", "lang": "en"}, {"value": "Globales Erwärmungspotenzial fossil (GWP-fossil)", "lang": "de"}], "type": "LCIA method data set", "refObjectId": "5f635281-343e-44fb-83df-1971b155e6b6", "uri": "../lciamethods/5f635281-343e-44fb-83df-1971b155e6b6.xml"}, "other": {"anies": [{"name": "referenceToUnitGroupDataSet", "value": {"shortDescription": [{"value": "kg CO_(2)-Äq.", "lang": "en"}], "type": "unit group data set", "refObjectId": "1ebf3012-d0db-4de2-aefd-ef30cedb0be1", "uri": "../unitgroups/1ebf3012-d0db-4de2-aefd-ef30cedb0be1.xml"}}, {"value": "1.5", "module": "A1-A3"}, {"value": "0.0281", "module": "A4"}, {"value": "0.0349", "module": "A5"}, {"value": "0.00064", "module": "C1"}, {"value": "0.00223", "module": "C2"}, {"value": "0", "module": "C3", "scenario": "S2"}, {"value": "0.00271", "module": "C3", "scenario": "S3"}, {"value": "0.0152", "module": "C4"}, {"value": "-0.0474", "module": "D", "scenario": "S0"}, {"value": "-1.5", "module": "D", "scenario": "S2"}, {"value": "-0.2", "module": "D", "scenario": "S3"}]}}, {"referenceToLCIAMethodDataSet": {"shortDescription": [{"value": "Global Warming Potential biogenic (GWP-biogenic)", "lang": "en"}, {"value": "Globales Erwärmungspotenzial biogen (GWP-biogenic)", "lang": "de"}], "type": "LCIA method data set", "refObjectId": "2356e1ab-0185-4db5-86e5-16de51c7485c", "uri": "../lciamethods/2356e1ab-0185-4db5-86e5-16de51c7485c.xml"}, "other": {"anies": [{"name": "referenceToUnitGroupDataSet", "value": {"shortDescription": [{"value": "kg CO_(2)-Äq.", "lang": "en"}], "type": "unit group data set", "refObjectId": "1ebf3012-d0db-4de2-aefd-ef30cedb0be1", "uri": "../unitgroups/1ebf3012-d0db-4de2-aefd-ef30cedb0be1.xml"}}, {"value": "-0.0631", "module": "A1-A3"}, {"value": "0.00134", "module": "A4"}, {"value": "0.0887", "module": "A5"}, {"value": "1.93E-06", "module": "C1"}, {"value": "0.000106", "module": "C2"}, {"value": "0", "module": "C3", "scenario": "S2"}, {"value": "2.38E-05", "module": "C3", "scenario": "S3"}, {"value": "4.86E-05", "module": "C4"}, {"value": "-0.00011", "module": "D", "scenario": "S0"}, {"value": "0.0631", "module": "D", "scenario": "S2"}, {"value": "-0.000315", "module": "D", "scenario": "S3"}]}}, {"referenceToLCIAMethodDataSet": {"shortDescription": [{"value": "Global Warming Potential luluc (GWP-luluc)", "lang": "en"}, {"value": "Globales Erwärmungspotenzial luluc (GWP-luluc)", "lang": "de"}], "type": "LCIA method data set", "refObjectId": "4331bbdb-978a-490d-8707-eeb047f01a55", "uri": "../lciamethods/4331bbdb-978a-490d-8707-eeb047f01a55.xml"}, "other": {"anies": [{"name": "referenceToUnitGroupDataSet", "value": {"shortDescription": [{"value": "kg CO_(2)-Äq.", "lang": "en"}], "type": "unit group data set", "refObjectId": "1ebf3012-d0db-4de2-aefd-ef30cedb0be1", "uri": "../unitgroups/1ebf3012-d0db-4de2-aefd-ef30cedb0be1.xml"}}, {"value": "0.00127", "module": "A1-A3"}, {"value": "0.000228", "module": "A4"}, {"value": "2.82E-06", "module": "A5"}, {"value": "4.99E-06", "module": "C1"}, {"value": "1.81E-05", "module": "C2"}, {"value": "0", "module": "C3", "scenario": "S2"}, {"value": "3.92E-06", "module": "C3", "scenario": "S3"}, {"value": "4.37E-05", "module": "C4"}, {"value": "-3.19E-05", "module": "D", "scenario": "S0"}, {"value": "-0.00127", "module": "D", "scenario": "S2"}, {"value": "-4.81E-05", "module": "D", "scenario": "S3"}]}}, {"referenceToLCIAMethodDataSet": {"shortDescription": [{"value": "Depletion potential of the stratospheric ozone layer (ODP)", "lang": "en"}, {"value": "Abbau Potential der stratosphärischen Ozonschicht (ODP)", "lang": "de"}], "type": "LCIA method data set", "refObjectId": "b5c629d6-def3-11e6-bf01-fe55135034f3", "uri": "../lciamethods/b5c629d6-def3-11e6-bf01-fe55135034f3.xml"}, "other": {"anies": [{"name": "referenceToUnitGroupDataSet", "value": {"shortDescription": [{"value": "kg CFC11-Äq.", "lang": "en"}], "type": "unit group data set", "refObjectId": "d9e957c9-7309-4474-bf3a-7777df6c4e5b", "uri": "../unitgroups/d9e957c9-7309-4474-bf3a-7777df6c4e5b.xml"}}, {"value": "7.38E-14", "module": "A1-A3"}, {"value": "3.39E-18", "module": "A4"}, {"value": "2.84E-17", "module": "A5"}, {"value": "7.41E-20", "module": "C1"}, {"value": "2.68E-19", "module": "C2"}, {"value": "0", "module": "C3", "scenario": "S2"}, {"value": "5.95E-17", "module": "C3", "scenario": "S3"}, {"value": "5.62E-17", "module": "C4"}, {"value": "-4.74E-16", "module": "D", "scenario": "S0"}, {"value": "-7.38E-14", "module": "D", "scenario": "S2"}, {"value": "-3.65E-16", "module": "D", "scenario": "S3"}]}}, {"referenceToLCIAMethodDataSet": {"shortDescription": [{"value": "Acidification potential of land and water (AP)", "lang": "en"}, {"value": "Versauerungspotenzial von Boden und Wasser (AP)", "lang": "de"}], "type": "LCIA method data set", "refObjectId": "b5c611c6-def3-11e6-bf01-fe55135034f3", "uri": "../lciamethods/b5c611c6-def3-11e6-bf01-fe55135034f3.xml"}, "other": {"anies": [{"name": "referenceToUnitGroupDataSet", "value": {"shortDescription": [{"value": "mol H^(+)-Äq.", "lang": "en"}], "type": "unit group data set", "refObjectId": "42e089ac-92bf-4bf2-8ca1-5fc40d18f2ed", "uri": "../unitgroups/42e089ac-92bf-4bf2-8ca1-5fc40d18f2ed.xml"}}, {"value": "0.0053", "module": "A1-A3"}, {"value": "2.96E-05", "module": "A4"}, {"value": "2.01E-05", "module": "A5"}, {"value": "3.09E-06", "module": "C1"}, {"value": "7.17E-06", "module": "C2"}, {"value": "0", "module": "C3", "scenario": "S2"}, {"value": "5.97E-06", "module": "C3", "scenario": "S3"}, {"value": "0.000109", "module": "C4"}, {"value": "-6.5E-05", "module": "D", "scenario": "S0"}, {"value": "-0.0053", "module": "D", "scenario": "S2"}, {"value": "-0.000186", "module": "D", "scenario": "S3"}]}}, {"referenceToLCIAMethodDataSet": {"shortDescription": [{"value": "Eutrophication potential aquatic freshwater (EP-freshwater)", "lang": "en"}, {"value": "Eutrophierungspotenzial Süßwasser (EP-freshwater)", "lang": "de"}], "type": "LCIA method data set", "refObjectId": "b53ec18f-7377-4ad3-86eb-cc3f4f276b2b", "uri": "../lciamethods/b53ec18f-7377-4ad3-86eb-cc3f4f276b2b.xml"}, "other": {"anies": [{"name": "referenceToUnitGroupDataSet", "value": {"shortDescription": [{"value": "kg PO_(4)-Äq.", "lang": "en"}], "type": "unit group data set", "refObjectId": "0429039d-a61d-4590-ba67-aa4a20a810a1", "uri": "../unitgroups/0429039d-a61d-4590-ba67-aa4a20a810a1.xml"}}, {"value": "1.49E-05", "module": "A1-A3"}, {"value": "8.57E-08", "module": "A4"}, {"value": "4.48E-09", "module": "A5"}, {"value": "1.87E-09", "module": "C1"}, {"value": "6.79E-09", "module": "C2"}, {"value": "0", "module": "C3", "scenario": "S2"}, {"value": "7.23E-09", "module": "C3", "scenario": "S3"}, {"value": "2.6E-08", "module": "C4"}, {"value": "-5.87E-08", "module": "D", "scenario": "S0"}, {"value": "-1.49E-05", "module": "D", "scenario": "S2"}, {"value": "-7.33E-08", "module": "D", "scenario": "S3"}]}}, {"referenceToLCIAMethodDataSet": {"shortDescription": [{"value": "Eutrophication potential aquatic marine (EP-marine)", "lang": "en"}, {"value": "Eutrophierungspotenzial Salzwasser (EP-marine)", "lang": "de"}], "type": "LCIA method data set", "refObjectId": "b5c619fa-def3-11e6-bf01-fe55135034f3", "uri": "../lciamethods/b5c619fa-def3-11e6-bf01-fe55135034f3.xml"}, "other": {"anies": [{"name": "referenceToUnitGroupDataSet", "value": {"shortDescription": [{"value": "kg N-Äq.", "lang": "en"}], "type": "unit group data set", "refObjectId": "d05bb823-ecdf-4686-8c40-bf1d9257859f", "uri": "../unitgroups/d05bb823-ecdf-4686-8c40-bf1d9257859f.xml"}}, {"value": "0.00159", "module": "A1-A3"}, {"value": "8.77E-06", "module": "A4"}, {"value": "6.05E-06", "module": "A5"}, {"value": "1.44E-06", "module": "C1"}, {"value": "3.23E-06", "module": "C2"}, {"value": "0", "module": "C3", "scenario": "S2"}, {"value": "1.33E-06", "module": "C3", "scenario": "S3"}, {"value": "2.8E-05", "module": "C4"}, {"value": "-1.69E-05", "module": "D", "scenario": "S0"}, {"value": "-0.00159", "module": "D", "scenario": "S2"}, {"value": "-6.66E-05", "module": "D", "scenario": "S3"}]}}, {"referenceToLCIAMethodDataSet": {"shortDescription": [{"value": "Eutrophication potential terrestrial (EP-terrestrial)", "lang": "en"}, {"value": "Eutrophierungspotenzial Land (EP-terrestrial)", "lang": "de"}], "type": "LCIA method data set", "refObjectId": "b5c614d2-def3-11e6-bf01-fe55135034f3", "uri": "../lciamethods/b5c614d2-def3-11e6-bf01-fe55135034f3.xml"}, "other": {"anies": [{"name": "referenceToUnitGroupDataSet", "value": {"shortDescription": [{"value": "mol N-Äq.", "lang": "en"}], "type": "unit group data set", "refObjectId": "71b4d617-0ec9-4d3f-b65e-e438940c2401", "uri": "../unitgroups/71b4d617-0ec9-4d3f-b65e-e438940c2401.xml"}}, {"value": "0.0183", "module": "A1-A3"}, {"value": "0.000105", "module": "A4"}, {"value": "9.35E-05", "module": "A5"}, {"value": "1.59E-05", "module": "C1"}, {"value": "3.61E-05", "module": "C2"}, {"value": "0", "module": "C3", "scenario": "S2"}, {"value": "1.39E-05", "module": "C3", "scenario": "S3"}, {"value": "0.000308", "module": "C4"}, {"value": "-0.000182", "module": "D", "scenario": "S0"}, {"value": "-0.0183", "module": "D", "scenario": "S2"}, {"value": "-0.000732", "module": "D", "scenario": "S3"}]}}, {"referenceToLCIAMethodDataSet": {"shortDescription": [{"value": "Formation potential of tropospheric ozone photochemical oxidants (POCP)", "lang": "en"}, {"value": "Bildungspotential für troposphärisches Ozon (POCP)", "lang": "de"}], "type": "LCIA method data set", "refObjectId": "b5c610fe-def3-11e6-bf01-fe55135034f3", "uri": "../lciamethods/b5c610fe-def3-11e6-bf01-fe55135034f3.xml"}, "other": {"anies": [{"name": "referenceToUnitGroupDataSet", "value": {"shortDescription": [{"value": "kg NMVOC-Äq.", "lang": "en"}], "type": "unit group data set", "refObjectId": "d27c25f8-fbc1-44c6-b47b-4adbae4199c6", "uri": "../unitgroups/d27c25f8-fbc1-44c6-b47b-4adbae4199c6.xml"}}, {"value": "0.00381", "module": "A1-A3"}, {"value": "2.41E-05", "module": "A4"}, {"value": "1.64E-05", "module": "A5"}, {"value": "4.03E-06", "module": "C1"}, {"value": "6.33E-06", "module": "C2"}, {"value": "0", "module": "C3", "scenario": "S2"}, {"value": "3.64E-06", "module": "C3", "scenario": "S3"}, {"value": "8.48E-05", "module": "C4"}, {"value": "-4.88E-05", "module": "D", "scenario": "S0"}, {"value": "-0.00381", "module": "D", "scenario": "S2"}, {"value": "-0.000201", "module": "D", "scenario": "S3"}]}}, {"referenceToLCIAMethodDataSet": {"shortDescription": [{"value": "Abiotic depletion potential for non fossil resources (ADPE)", "lang": "en"}, {"value": "Potenzial für den abiotischen Abbau nicht fossiler Ressourcen (ADPE)", "lang": "de"}], "type": "LCIA method data set", "refObjectId": "b2ad6494-c78d-11e6-9d9d-cec0c932ce01", "uri": "../lciamethods/b2ad6494-c78d-11e6-9d9d-cec0c932ce01.xml"}, "other": {"anies": [{"name": "referenceToUnitGroupDataSet", "value": {"shortDescription": [{"value": "kg Sb-Äq.", "lang": "en"}], "type": "unit group data set", "refObjectId": "54ccd2d9-a32a-4fc2-923d-f2c8c93e89d4", "uri": "../unitgroups/54ccd2d9-a32a-4fc2-923d-f2c8c93e89d4.xml"}}, {"value": "2.05E-07", "module": "A1-A3"}, {"value": "2.02E-09", "module": "A4"}, {"value": "4.14E-10", "module": "A5"}, {"value": "4.42E-11", "module": "C1"}, {"value": "1.6E-10", "module": "C2"}, {"value": "0", "module": "C3", "scenario": "S2"}, {"value": "7.83E-10", "module": "C3", "scenario": "S3"}, {"value": "1.36E-09", "module": "C4"}, {"value": "-7.56E-09", "module": "D", "scenario": "S0"}, {"value": "-2.05E-07", "module": "D", "scenario": "S2"}, {"value": "-1.42E-08", "module": "D", "scenario": "S3"}]}}, {"referenceToLCIAMethodDataSet": {"shortDescription": [{"value": "Abiotic depletion potential for fossil resources (ADPF)", "lang": "en"}, {"value": "Potenzial für den abiotischen Abbau fossiler Brennstoffe (ADPF)", "lang": "de"}], "type": "LCIA method data set", "refObjectId": "b2ad6110-c78d-11e6-9d9d-cec0c932ce01", "uri": "../lciamethods/b2ad6110-c78d-11e6-9d9d-cec0c932ce01.xml"}, "other": {"anies": [{"name": "referenceToUnitGroupDataSet", "value": {"shortDescription": [{"value": "MJ", "lang": "en"}], "type": "unit group data set", "refObjectId": "93a60a57-a3c8-11da-a746-0800200c9a66", "uri": "../unitgroups/93a60a57-a3c8-11da-a746-0800200c9a66.xml"}}, {"value": "21.8", "module": "A1-A3"}, {"value": "0.376", "module": "A4"}, {"value": "0.0358", "module": "A5"}, {"value": "0.0082", "module": "C1"}, {"value": "0.0297", "module": "C2"}, {"value": "0", "module": "C3", "scenario": "S2"}, {"value": "0.0476", "module": "C3", "scenario": "S3"}, {"value": "0.199", "module": "C4"}, {"value": "-0.804", "module": "D", "scenario": "S0"}, {"value": "-21.8", "module": "D", "scenario": "S2"}, {"value": "-3.29", "module": "D", "scenario": "S3"}]}}, {"referenceToLCIAMethodDataSet": {"shortDescription": [{"value": "Water use (WDP)", "lang": "en"}, {"value": "Wassernutzung (WDP)", "lang": "de"}], "type": "LCIA method data set", "refObjectId": "b2ad66ce-c78d-11e6-9d9d-cec0c932ce01", "uri": "../lciamethods/b2ad66ce-c78d-11e6-9d9d-cec0c932ce01.xml"}, "other": {"anies": [{"name": "referenceToUnitGroupDataSet", "value": {"shortDescription": [{"value": "m^(3) world-Äq. deprived", "lang": "en"}], "type": "unit group data set", "refObjectId": "6ae2df01-888e-46c8-b17d-49fa3869b476", "uri": "../unitgroups/6ae2df01-888e-46c8-b17d-49fa3869b476.xml"}}, {"value": "0.126", "module": "A1-A3"}, {"value": "0.000252", "module": "A4"}, {"value": "0.0129", "module": "A5"}, {"value": "5.51E-06", "module": "C1"}, {"value": "2E-05", "module": "C2"}, {"value": "0", "module": "C3", "scenario": "S2"}, {"value": "0.00059", "module": "C3", "scenario": "S3"}, {"value": "0.00159", "module": "C4"}, {"value": "-0.00471", "module": "D", "scenario": "S0"}, {"value": "-0.126", "module": "D", "scenario": "S2"}, {"value": "-0.00371", "module": "D", "scenario": "S3"}]}}, {"referenceToLCIAMethodDataSet": {"shortDescription": [{"value": "Incidence of disease due to PM emissions (PM)", "lang": "en"}, {"value": "Auftreten von Krankheiten aufgrund von Feinstaubemissionen (PM)", "lang": "de"}], "type": "LCIA method data set", "refObjectId": "b5c602c6-def3-11e6-bf01-fe55135034f3", "uri": "../lciamethods/b5c602c6-def3-11e6-bf01-fe55135034f3.xml"}, "other": {"anies": [{"name": "referenceToUnitGroupDataSet", "value": {"shortDescription": [{"value": "Disease incidence", "lang": "en"}], "type": "unit group data set", "refObjectId": "3883559b-648f-4afc-8ba2-0bd24f3affa3", "uri": "../unitgroups/3883559b-648f-4afc-8ba2-0bd24f3affa3.xml"}}, {"value": "5.9E-08", "module": "A1-A3"}, {"value": "1.73E-10", "module": "A4"}, {"value": "1.49E-10", "module": "A5"}, {"value": "3.47E-11", "module": "C1"}, {"value": "3.92E-11", "module": "C2"}, {"value": "0", "module": "C3", "scenario": "S2"}, {"value": "5.01E-11", "module": "C3", "scenario": "S3"}, {"value": "1.35E-09", "module": "C4"}, {"value": "-5.52E-10", "module": "D", "scenario": "S0"}, {"value": "-5.9E-08", "module": "D", "scenario": "S2"}, {"value": "-9.95E-09", "module": "D", "scenario": "S3"}]}}, {"referenceToLCIAMethodDataSet": {"shortDescription": [{"value": "Human exposure efficiency relative to U235 (IR)", "lang": "en"}, {"value": "Wirkung durch Exposition des Menschen mit U235 (IR)", "lang": "de"}], "type": "LCIA method data set", "refObjectId": "b5c632be-def3-11e6-bf01-fe55135034f3", "uri": "../lciamethods/b5c632be-def3-11e6-bf01-fe55135034f3.xml"}, "other": {"anies": [{"name": "referenceToUnitGroupDataSet", "value": {"shortDescription": [{"value": "kBq U235-Äq.", "lang": "en"}], "type": "unit group data set", "refObjectId": "456b05bf-1415-44a9-9993-02452f554c09", "uri": "../unitgroups/456b05bf-1415-44a9-9993-02452f554c09.xml"}}, {"value": "0.0135", "module": "A1-A3"}, {"value": "6.73E-05", "module": "A4"}, {"value": "0.000233", "module": "A5"}, {"value": "1.47E-06", "module": "C1"}, {"value": "5.33E-06", "module": "C2"}, {"value": "0", "module": "C3", "scenario": "S2"}, {"value": "0.00118", "module": "C3", "scenario": "S3"}, {"value": "0.000232", "module": "C4"}, {"value": "-0.00943", "module": "D", "scenario": "S0"}, {"value": "-0.0135", "module": "D", "scenario": "S2"}, {"value": "-0.00719", "module": "D", "scenario": "S3"}]}}, {"referenceToLCIAMethodDataSet": {"shortDescription": [{"value": "Comparative toxic unit for ecosystems (ETP-fw)", "lang": "en"}, {"value": "Toxizitätsvergleichseinheit für Ökosysteme (ETP-fw)", "lang": "de"}], "type": "LCIA method data set", "refObjectId": "ee1082d1-b0f7-43ca-a1f0-21e2a4a74511", "uri": "../lciamethods/ee1082d1-b0f7-43ca-a1f0-21e2a4a74511.xml"}, "other": {"anies": [{"name": "referenceToUnitGroupDataSet", "value": {"shortDescription": [{"value": "CTUe", "lang": "en"}], "type": "unit group data set", "refObjectId": "aa959ded-f1eb-4efb-9c5c-2d60be36b3e6", "uri": "../unitgroups/aa959ded-f1eb-4efb-9c5c-2d60be36b3e6.xml"}}, {"value": "47.1", "module": "A1-A3"}, {"value": "0.265", "module": "A4"}, {"value": "0.0148", "module": "A5"}, {"value": "0.0058", "module": "C1"}, {"value": "0.021", "module": "C2"}, {"value": "0", "module": "C3", "scenario": "S2"}, {"value": "0.0203", "module": "C3", "scenario": "S3"}, {"value": "0.114", "module": "C4"}, {"value": "-0.167", "module": "D", "scenario": "S0"}, {"value": "-47.1", "module": "D", "scenario": "S2"}, {"value": "-0.181", "module": "D", "scenario": "S3"}]}}, {"referenceToLCIAMethodDataSet": {"shortDescription": [{"value": "Comparative toxic unit for humans (carcinogenic) (HTP-c)", "lang": "en"}, {"value": "Toxizitätsvergleichseinheit für Menschen (krebserregend) (HTP-c)", "lang": "de"}], "type": "LCIA method data set", "refObjectId": "2299222a-bbd8-474f-9d4f-4dd1f18aea7c", "uri": "../lciamethods/2299222a-bbd8-474f-9d4f-4dd1f18aea7c.xml"}, "other": {"anies": [{"name": "referenceToUnitGroupDataSet", "value": {"shortDescription": [{"value": "CTUh", "lang": "en"}], "type": "unit group data set", "refObjectId": "d4c9523e-2d7e-49fd-8469-998f547d3a70", "uri": "../unitgroups/d4c9523e-2d7e-49fd-8469-998f547d3a70.xml"}}, {"value": "5.79E-10", "module": "A1-A3"}, {"value": "5.56E-12", "module": "A4"}, {"value": "1.08E-12", "module": "A5"}, {"value": "1.21E-13", "module": "C1"}, {"value": "4.4E-13", "module": "C2"}, {"value": "0", "module": "C3", "scenario": "S2"}, {"value": "5.62E-13", "module": "C3", "scenario": "S3"}, {"value": "1.68E-11", "module": "C4"}, {"value": "-7.43E-12", "module": "D", "scenario": "S0"}, {"value": "-5.79E-10", "module": "D", "scenario": "S2"}, {"value": "-2.46E-11", "module": "D", "scenario": "S3"}]}}, {"referenceToLCIAMethodDataSet": {"shortDescription": [{"value": "Comparative toxic unit for humans (noncarcinogenic) (HTP-nc)", "lang": "en"}, {"value": "Toxizitätsvergleichseinheit für Menschen (nicht krebserregend) (HTP-nc)", "lang": "de"}], "type": "LCIA method data set", "refObjectId": "3af763a5-b7a1-48c9-9cee-1f223481fcef", "uri": "../lciamethods/3af763a5-b7a1-48c9-9cee-1f223481fcef.xml"}, "other": {"anies": [{"name": "referenceToUnitGroupDataSet", "value": {"shortDescription": [{"value": "CTUh", "lang": "en"}], "type": "unit group data set", "refObjectId": "d4c9523e-2d7e-49fd-8469-998f547d3a70", "uri": "../unitgroups/d4c9523e-2d7e-49fd-8469-998f547d3a70.xml"}}, {"value": "2.21E-08", "module": "A1-A3"}, {"value": "2.88E-10", "module": "A4"}, {"value": "7.17E-11", "module": "A5"}, {"value": "7.28E-12", "module": "C1"}, {"value": "2.58E-11", "module": "C2"}, {"value": "0", "module": "C3", "scenario": "S2"}, {"value": "2.07E-11", "module": "C3", "scenario": "S3"}, {"value": "1.86E-09", "module": "C4"}, {"value": "-2.76E-10", "module": "D", "scenario": "S0"}, {"value": "-2.21E-08", "module": "D", "scenario": "S2"}, {"value": "-9.43E-10", "module": "D", "scenario": "S3"}]}}, {"referenceToLCIAMethodDataSet": {"shortDescription": [{"value": "Soil quality index (SQP)", "lang": "en"}, {"value": "Bodenqualitätsindex (SQP)", "lang": "de"}], "type": "LCIA method data set", "refObjectId": "b2ad6890-c78d-11e6-9d9d-cec0c932ce01", "uri": "../lciamethods/b2ad6890-c78d-11e6-9d9d-cec0c932ce01.xml"}, "other": {"anies": [{"name": "referenceToUnitGroupDataSet", "value": {"shortDescription": [{"value": "SQP", "lang": "en"}], "type": "unit group data set", "refObjectId": "f130951c-e67f-4f7f-8dd4-665de3974e18", "uri": "../unitgroups/f130951c-e67f-4f7f-8dd4-665de3974e18.xml"}}, {"value": "30.4", "module": "A1-A3"}, {"value": "0.132", "module": "A4"}, {"value": "0.0102", "module": "A5"}, {"value": "0.00288", "module": "C1"}, {"value": "0.0104", "module": "C2"}, {"value": "0", "module": "C3", "scenario": "S2"}, {"value": "0.0151", "module": "C3", "scenario": "S3"}, {"value": "0.0415", "module": "C4"}, {"value": "-0.121", "module": "D", "scenario": "S0"}, {"value": "-30.4", "module": "D", "scenario": "S2"}, {"value": "-0.107", "module": "D", "scenario": "S3"}]}}]}, "otherAttributes": {"{http://www.indata.network/EPD/2019}epd-version": "1.2"}, "version": "1.1", "locations": "../ILCDLocations.xml"}