{"processInformation": {"dataSetInformation": {"UUID": "f2100a64-5daf-4650-a3e6-b7be47036d64", "name": {"baseName": [{"value": "Geryon Security Revolving Door", "lang": "en"}, {"value": "Geryon Sicherheits-Drehtür", "lang": "de"}], "functionalUnitFlowProperties": [{"lang": "en"}]}, "classificationInformation": {"classification": [{"class": [{"value": "Komponenten von Fenstern und Vorhangfassaden", "level": 0, "classId": "7"}, {"value": "Türen und Tore", "level": 1, "classId": "7.6"}, {"value": "Aluminium", "level": 2, "classId": "7.6.02"}], "name": "OEKOBAU.DAT"}, {"class": [{"value": "02 Building products", "level": 0}, {"value": "Doors, windows, shutters, and related products", "level": 1}, {"value": "Electronic and physical Access Control Systems", "level": 2}], "name": "IBUCategories"}]}, "generalComment": [{"value": "Secure areas require a reliable system for identifying and separating authorized persons.\nAs these areas are usually representative of the building, a secure but at the same time transparent access solution is preferred.\n\nGeryon Security Revolving Door\nOwing to the high transparency grade of the glass elements and a wide variety of colours for the metal parts, all models elegantly blend in with their surroundings. A sophisticated sensor system in compliance with the latest standards prevents users from being injured.\nDepending on the security requirements, the door may be equipped with a contact mat, scales or internal monitoring. Other variants are reinforced bullet- and burglar-resistant designs, which are certified according to standards RC2 and RC3 respectively. Options like a rotating unit with an emergency exit function or a night closure complete the product range.", "lang": "en"}, {"value": "Sichere Bereiche erfordern ein zuverlässiges System zur Identifizierung und Trennung autorisierter Personen. Da diese Bereiche in der Regel repräsentativ für das Gebäude sind, wird eine sichere und gleichzeitig transparente Zugangslösung bevorzugt. Geryon Sicherheitskarusselltür Dank des hohen Transparenzgrades der Glaselemente und einer großen Farbvielfalt der Metallteile fügen sich alle Modelle elegant in ihre Umgebung ein. Ein ausgeklügeltes Sensorsystem, das den neuesten Standards entspricht, verhindert, dass Benutzer verletzt werden. Je nach Sicherheitsanforderungen kann die Tür mit einer Kontaktmatte, einer Waage oder einer internen Überwachung ausgestattet werden. Weitere Varianten sind verstärkte kugelsichere und einbruchhemmende Ausführungen, die nach den Normen RC2 bzw. RC3 zertifiziert sind. Optionen wie eine Dreheinheit mit Notausgangsfunktion oder ein Nachtverschluss runden die Produktpalette ab.", "lang": "de"}]}, "quantitativeReference": {"referenceToReferenceFlow": [0]}, "time": {"referenceYear": 2024, "dataSetValidUntil": 2027, "other": {"anies": [{"name": "publicationDateOfEPD", "value": 1709251200000}]}}, "geography": {"locationOfOperationSupplyOrProduction": {"location": "DE"}}, "technology": {"technologyDescriptionAndIncludedProcesses": [{"value": "Thanks to the high degree of transparency of the glass elements and the wide range of colours of the metal parts, all models blend elegantly into their surroundings. Sophisticated sensor technology in accordance with the latest standards prevents users from being injured. Depending on security requirements, the door can be fitted with a contact mat, a scale or internal monitoring. Other variants include reinforced bullet and burglar-resistant versions that are certified to RC2 and RC3 standards. Options such as a turn unit with emergency exit function or a night lock round off the product range. \nTechnical data: \nKey elements and options of the Geryon Security Revolving Door:\n\n• Users cannot become stuck thanks to end point locking\n• Safety sensor system according to DIN EN 16005\n• Standard version has IR sensor system\n• Versions with resistance classes RC2 and RC3\n• All-glass units with underfloor drive\n• Option with approved emergency exit column\n• Option with in-built scales with weight limits or actual weight\n• Option with night closure\n• Option with optical separation using SRD Vision\n\nFollowing technical data apply for Geryon Security Revolving Door (SRD-E01): \nDeclared unit: \nThe declared unit is 1 piece of product: 459 kg", "lang": "en"}, {"value": "Dank der hohen Transparenz der Glaselemente und der großen Farbvielfalt der Metallteile fügen sich alle Modelle elegant in ihre Umgebung ein. Eine ausgefeilte Sensorik nach neuesten Standards verhindert, dass der Nutzer verletzt wird. Je nach Sicherheitsbedürfnis kann die Tür mit einer Kontaktmatte, einer Waage oder einer Innenüberwachung ausgestattet werden. Weitere Varianten sind verstärkte kugelsichere und einbruchhemmende Ausführungen, die nach den Normen RC2 und RC3 zertifiziert sind. Optionen wie eine Dreheinheit mit Notausgangsfunktion oder eine Nachtverriegelung runden die Produktpalette ab. \nTechnische Daten: \nSchlüsselelemente und Optionen der Geryon Sicherheitskarusselltür: - Kein Einklemmen des Benutzers dank Endpunktverriegelung - Sicherheitssensorik nach DIN EN 16005 - Standardausführung mit IR-Sensorik - Ausführungen mit Widerstandsklassen RC2 und RC3 - Ganzglasanlagen mit Unterflurantrieb - Option mit zugelassener Notausgangssäule - Option mit eingebauter Waage mit Gewichtsbegrenzung oder Ist-Gewicht - Option mit Nachtverschluss - Option mit optischer Trennung durch SRD Vision Für die Geryon Sicherheitskarusselltür (SRD-E01) gelten folgende technische Daten: \nDeklarierte Einheit: \nDie angegebene Einheit ist 1 Stück des Produkts: 459 kg", "lang": "de"}], "technologicalApplicability": [{"value": "For secure entry to:\n\nSensitive areas in administrative buildings,\nindustrial premises, government agencies and\nministries\nBanks and financial institutions\nData and research centres\nStaff entrances at airports\nNuclear power plants", "lang": "en"}, {"value": "Für den sicheren Zugang zu: Sensiblen Bereichen in Verwaltungsgebäuden, Industrieanlagen, Behörden und Ministerien Banken und Finanzinstituten Daten- und Forschungszentren Personaleingänge an Flughäfen Kernkraftwerke", "lang": "de"}]}}, "modellingAndValidation": {"LCIMethodAndAllocation": {"typeOfDataSet": "EPD", "referenceToLCAMethodDetails": [{"shortDescription": [{"value": "Electronic and physical Access Control Systems.pdf", "lang": "en"}], "type": "source data set", "refObjectId": "9beaca90-3d2f-485e-aa6b-5611d678b941"}], "other": {"anies": [{"name": "subType", "value": "specific dataset"}]}}, "dataSourcesTreatmentAndRepresentativeness": {"referenceToDataSource": [{"shortDescription": [{"value": "GaBi Database (all versions)", "lang": "en"}], "type": "source data set", "refObjectId": "28d74cc0-db8b-4d7e-bc44-5f6d56ce0c4a"}, {"shortDescription": [{"value": "GaBi Database Edition 2021, CUP 2021.01", "lang": "en"}], "type": "source data set", "refObjectId": "1cece811-7501-44d4-8067-9259bd5cb835"}], "useAdviceForDataSet": [{"value": "Scope: \nThis Environmental Product Declaration refers to a specific Geryon Security Revolving Door (SRD-E01) covering the variants 120° and 180°. The products are manufactured at the dormakaba production facility in Bhl (Germany).\nGreen electricity is being used at this production site.\n\nData represents the year 2022. \nSystem boundary: \nType of EPD: cradle to gate with options, modules C1–C4, and module D (A1–A3 + C + D and additional modules: A4 + A5 + B6)\n\nProduction - Module A1-A3\nThe product stage includes: \n— A1, raw material extraction, processing and mechanical treatments, processing of secondary material input (e.g. recycling processes), — A2, transport to the manufacturer, \n— A3, manufacturing and assembly including provision of all materials, products and energy, as well as waste processing up to the end-of-waste state.\n\nConstruction stage - Modules A4-A5\nThe construction process stage includes: \n— A4, transport to the building site; \n— A5, installation into the building; \nincluding provision of all materials, products and energy, as well as waste processing up to the end-of-waste state or disposal of final residues during the construction process stage.\n\nUse stage - Module B6\nThe use stage related to the operation of the building includes: \n— B6, operational energy use. \nThe potential use of electricity from the grid is declared in module B6.\n\nEnd-of-life stage– Modules C1-C4 and D\nThe end-of-life stage includes: \n— C1, de-construction, demolition: \n— C2, transport to waste processing; \n— C3, waste processing for reuse, recovery and/or recycling; \n— C4, disposal; \nincluding provision and all transport, provision of all materials, products and related energy and water use. \n\nModule D (Benefits and loads beyond the system boundary) includes: \n— D, recycling potentials, expressed as net impacts and benefits.", "lang": "en"}, {"value": "Gültigkeitsbereich: \nDiese Umweltproduktdeklaration bezieht sich auf eine bestimmte Geryon Sicherheitskarusselltür (SRD-E01) in den Varianten 120° und 180°. Die Produkte werden in der dormakaba Produktionsstätte in Bühl (Deutschland) hergestellt. An diesem Produktionsstandort wird Ökostrom verwendet. Die Daten beziehen sich auf das Jahr 2022. \nSystemgrenze: \nArt der EPD: Cradle to Gate mit Optionen, Modulen C1-C4 und Modul D (A1-A3 + C + D und zusätzliche Module: A4 + A5 + B6) Produktion - Modul A1-A3 Die Produktphase umfasst: - A1, Rohstoffgewinnung, Verarbeitung und mechanische Bearbeitung, Verarbeitung von Sekundärmaterial (z.B. Recyclingprozesse), - A2, Transport zum Hersteller, - A3, Fertigung und Montage einschließlich der Bereitstellung aller Materialien, Produkte und Energie sowie die Abfallverarbeitung bis zum End-of-Waste-Zustand. Bauphase - Module A4-A5 Die Bauprozessphase umfasst: - A4, Transport zur Baustelle; - A5, Einbau in das Gebäude; einschließlich der Bereitstellung aller Materialien, Produkte und Energie sowie der Abfallverarbeitung bis zum Ende des Abfallzustands oder der Entsorgung der endgültigen Rückstände während der Bauprozessphase. Nutzungsphase - Modul B6 Die Nutzungsphase im Zusammenhang mit dem Betrieb des Gebäudes umfasst: - B6, Betriebliche Energienutzung. Die mögliche Nutzung von Strom aus dem Netz wird in Modul B6 angegeben. End-of-Life-Stadium - Module C1-C4 und D Das End-of-Life-Stadium umfasst: - C1, Rückbau, Abriss; - C2, Transport zur Abfallverarbeitung; - C3, Abfallverarbeitung zur Wiederverwendung, Verwertung und/oder zum Recycling; - C4, Entsorgung; einschließlich Bereitstellung und sämtlicher Transporte, Bereitstellung aller Materialien, Produkte und des damit verbundenen Energie- und Wasserverbrauchs. Modul D (Nutzen und Lasten jenseits der Systemgrenze) umfasst: - D, Recyclingpotenziale, ausgedrückt als Nettoauswirkungen und Nutzen.", "lang": "de"}], "other": {"anies": [{"name": "referenceToOriginalEPD", "value": {"shortDescription": {"value": "Geryon Security Revolving Door.pdf", "defaultValue": "Geryon Security Revolving Door.pdf", "lstrings": [{"lang": "en", "value": "Geryon Security Revolving Door.pdf"}]}, "type": "source data set", "uuid": {"uuid": "814a3ccc-fe6d-49d8-b833-74ae6cdd5829"}, "refObjectId": "814a3ccc-fe6d-49d8-b833-74ae6cdd5829", "resourceURLs": ["https://oekobaudat.de/OEKOBAU.DAT/resource/sources/814a3ccc-fe6d-49d8-b833-74ae6cdd5829/Geryon_Security_Revolving_Door_22795.pdf?version=00.02.000"]}}]}}, "validation": {"review": [{"referenceToNameOfReviewerAndInstitution": [{"shortDescription": [{"value": "Institut Bauen und Umwelt e. V.", "lang": "en"}], "type": "contact data set", "refObjectId": "d111dbec-b024-4be5-86c5-752d6eb2cf95", "uri": "../contacts/d111dbec-b024-4be5-86c5-752d6eb2cf95.xml"}], "type": "Accredited third party review"}]}, "complianceDeclarations": {"compliance": [{"referenceToComplianceSystem": {"shortDescription": [{"value": "DIN EN 15804+A2", "lang": "en"}], "type": "source data set", "refObjectId": "c0016b33-8cf7-415c-ac6e-deba0d21440d", "uri": "../sources/c0016b33-8cf7-415c-ac6e-deba0d21440d.xml"}}, {"referenceToComplianceSystem": {"shortDescription": [{"value": "ISO 14025", "lang": "en"}], "type": "source data set", "refObjectId": "4f2eb655-6e44-4874-a95a-e28f5442cd4d", "uri": "../sources/4f2eb655-6e44-4874-a95a-e28f5442cd4d.xml"}}]}}, "administrativeInformation": {"commissionerAndGoal": {"referenceToCommissioner": [{"shortDescription": [{"value": "dormakaba International Holding GmbH", "lang": "en"}], "type": "contact data set", "refObjectId": "33313944-7b37-498a-b458-25a295c1017d", "uri": "../contacts/33313944-7b37-498a-b458-25a295c1017d.xml"}]}, "dataGenerator": {"referenceToPersonOrEntityGeneratingTheDataSet": [{"shortDescription": [{"value": "dormakaba International Holding GmbH", "lang": "en"}], "type": "contact data set", "refObjectId": "33313944-7b37-498a-b458-25a295c1017d", "uri": "../contacts/33313944-7b37-498a-b458-25a295c1017d.xml"}]}, "dataEntryBy": {"timeStamp": 1709251200000, "referenceToDataSetFormat": [{"shortDescription": [{"value": "ILCD Format", "lang": "en"}], "type": "source data set", "refObjectId": "a97a0155-0234-4b87-b4ce-a45da52f2a40", "uri": "../sources/a97a0155-0234-4b87-b4ce-a45da52f2a40.xml"}, {"shortDescription": [{"value": "EPD-Datenformaterweiterungen v1.2", "lang": "de"}, {"value": "EPD Data Format Extensions v1.2", "lang": "en"}], "type": "source data set", "refObjectId": "a29449fd-aa2f-4de8-b5d7-4b06b43c6fde", "uri": "../sources/a29449fd-aa2f-4de8-b5d7-4b06b43c6fde.xml"}]}, "publicationAndOwnership": {"dataSetVersion": "00.05.000", "referenceToRegistrationAuthority": {"shortDescription": [{"value": "Institut Bauen und Umwelt e. V.", "lang": "en"}], "type": "contact data set", "refObjectId": "d111dbec-b024-4be5-86c5-752d6eb2cf95", "uri": "../contacts/d111dbec-b024-4be5-86c5-752d6eb2cf95.xml"}, "registrationNumber": "EPD-DOR-20240049-CBA2-EN", "referenceToOwnershipOfDataSet": {"shortDescription": [{"value": "dormakaba International Holding GmbH", "lang": "en"}], "type": "contact data set", "refObjectId": "33313944-7b37-498a-b458-25a295c1017d", "uri": "../contacts/33313944-7b37-498a-b458-25a295c1017d.xml"}, "copyright": true, "licenseType": "Free of charge for all users and uses", "accessRestrictions": [{"value": "None", "lang": "en"}], "other": {"anies": [{"name": "referenceToPublisher", "value": {"shortDescription": [{"value": "Institut Bauen und Umwelt e. V.", "lang": "en"}], "type": "contact data set", "refObjectId": "d111dbec-b024-4be5-86c5-752d6eb2cf95", "uri": "../contacts/d111dbec-b024-4be5-86c5-752d6eb2cf95.xml"}}]}}}, "exchanges": {"exchange": [{"dataSetInternalID": 0, "referenceToFlowDataSet": {"shortDescription": [{"value": "Geryon Security Revolving Door (Geryon Sicherheits-Drehtür)", "lang": "en"}], "type": "flow data set", "refObjectId": "b268a3f9-0069-9b2f-2078-87242f789b7f", "uri": "../flows/b268a3f9-0069-9b2f-2078-87242f789b7f.xml"}, "meanAmount": 1.0, "referencesToDataSource": {}, "referenceFlow": true, "resolvedFlowVersion": "00.05.000", "resultingflowAmount": 1.0, "flowProperties": [{"name": [{"lang": "en", "value": "Weight"}], "uuid": "93a60a56-a3c8-11da-a746-0800200b9a66", "meanValue": 459.0}, {"name": [{"lang": "de", "value": "Anzahl"}, {"lang": "en", "value": "Number of pieces"}], "uuid": "01846770-4cfe-4a25-8ad9-919d8d378345", "referenceFlowProperty": true, "meanValue": 1.0, "referenceUnit": "pcs.", "unitGroupUUID": "934110e3-baf4-49e9-992c-3d8109a6aafb"}], "materialProperties": [{"name": "weight per piece", "value": "459.0", "unit": "kg"}], "typeOfFlow": "Product flow", "classification": {"classHierarchy": "Komponenten von Fenstern und Vorhangfassaden / Türen und Tore / Aluminium", "name": "OEKOBAU.DAT"}}, {"dataSetInternalID": 1, "referenceToFlowDataSet": {"shortDescription": [{"value": "Renewable primary energy as energy carrier (PERE)", "lang": "en"}, {"value": "Erneuerbare Primärenergie als Energieträger (PERE)", "lang": "de"}], "type": "flow data set", "refObjectId": "20f32be5-0398-4288-9b6d-accddd195317", "uri": "../flows/20f32be5-0398-4288-9b6d-accddd195317.xml"}, "exchange direction": "INPUT", "other": {"anies": [{"name": "referenceToUnitGroupDataSet", "value": {"shortDescription": [{"value": "MJ", "lang": "en"}], "type": "unit group data set", "refObjectId": "93a60a57-a3c8-11da-a746-0800200c9a66", "uri": "../unitgroups/93a60a57-a3c8-11da-a746-0800200c9a66.xml"}}, {"value": "8681.802", "module": "A1-A3"}, {"value": "0.173", "module": "A4"}, {"value": "48.325", "module": "A5"}, {"value": "0", "module": "B2"}, {"value": "8218.1", "module": "B6"}, {"value": "0", "module": "C1"}, {"value": "0.086", "module": "C2"}, {"value": "17.307", "module": "C3"}, {"value": "4.96", "module": "C4"}, {"value": "-6287.3", "module": "D"}]}, "resolvedFlowVersion": "38.00.000", "flowProperties": [], "typeOfFlow": "Other flow", "classification": {"classHierarchy": "Quantities", "name": "GaBiCategories"}}, {"dataSetInternalID": 2, "referenceToFlowDataSet": {"shortDescription": [{"value": "Renewable primary energy resources as material utilization (PERM)", "lang": "en"}, {"value": "Erneuerbare Primärenergie zur stofflichen Nutzung (PERM)", "lang": "de"}], "type": "flow data set", "refObjectId": "fb3ec0de-548d-4508-aea5-00b73bf6f702", "uri": "../flows/fb3ec0de-548d-4508-aea5-00b73bf6f702.xml"}, "exchange direction": "INPUT", "other": {"anies": [{"name": "referenceToUnitGroupDataSet", "value": {"shortDescription": [{"value": "MJ", "lang": "en"}], "type": "unit group data set", "refObjectId": "93a60a57-a3c8-11da-a746-0800200c9a66", "uri": "../unitgroups/93a60a57-a3c8-11da-a746-0800200c9a66.xml"}}, {"value": "57.242", "module": "A1-A3"}, {"value": "0", "module": "A4"}, {"value": "-48", "module": "A5"}, {"value": "0", "module": "B2"}, {"value": "0", "module": "B6"}, {"value": "0", "module": "C1"}, {"value": "0", "module": "C2"}, {"value": "-9.242", "module": "C3"}, {"value": "0", "module": "C4"}, {"value": "0", "module": "D"}]}, "resolvedFlowVersion": "38.00.000", "flowProperties": [], "typeOfFlow": "Other flow", "classification": {"classHierarchy": "Quantities", "name": "GaBiCategories"}}, {"dataSetInternalID": 3, "referenceToFlowDataSet": {"shortDescription": [{"value": "Total use of renewable primary energy resources (PERT)", "lang": "en"}, {"value": "Total erneuerbare Primärenergie (PERT)", "lang": "de"}], "type": "flow data set", "refObjectId": "53f97275-fa8a-4cdd-9024-65936002acd0", "uri": "../flows/53f97275-fa8a-4cdd-9024-65936002acd0.xml"}, "exchange direction": "INPUT", "other": {"anies": [{"name": "referenceToUnitGroupDataSet", "value": {"shortDescription": [{"value": "MJ", "lang": "en"}], "type": "unit group data set", "refObjectId": "93a60a57-a3c8-11da-a746-0800200c9a66", "uri": "../unitgroups/93a60a57-a3c8-11da-a746-0800200c9a66.xml"}}, {"value": "8739.002", "module": "A1-A3"}, {"value": "0.173", "module": "A4"}, {"value": "0.325", "module": "A5"}, {"value": "0", "module": "B2"}, {"value": "8218.1", "module": "B6"}, {"value": "0", "module": "C1"}, {"value": "0.086", "module": "C2"}, {"value": "8.066", "module": "C3"}, {"value": "4.96", "module": "C4"}, {"value": "-6287.3", "module": "D"}]}, "resolvedFlowVersion": "38.00.000", "flowProperties": [], "typeOfFlow": "Other flow", "classification": {"classHierarchy": "Quantities / Environmental quantities / EPD EN 15804 / LCI indicators", "name": "GaBiCategories"}}, {"dataSetInternalID": 4, "referenceToFlowDataSet": {"shortDescription": [{"value": "Non renewable primary energy as energy carrier (PENRE)", "lang": "en"}, {"value": "Nicht-erneuerbare Primärenergie als Energieträger (PENRE)", "lang": "de"}], "type": "flow data set", "refObjectId": "ac857178-2b45-46ec-892a-a9a4332f0372", "uri": "../flows/ac857178-2b45-46ec-892a-a9a4332f0372.xml"}, "exchange direction": "INPUT", "other": {"anies": [{"name": "referenceToUnitGroupDataSet", "value": {"shortDescription": [{"value": "MJ", "lang": "en"}], "type": "unit group data set", "refObjectId": "93a60a57-a3c8-11da-a746-0800200c9a66", "uri": "../unitgroups/93a60a57-a3c8-11da-a746-0800200c9a66.xml"}}, {"value": "26138.51", "module": "A1-A3"}, {"value": "55.057", "module": "A4"}, {"value": "1.791", "module": "A5"}, {"value": "0", "module": "B2"}, {"value": "18545", "module": "B6"}, {"value": "0", "module": "C1"}, {"value": "27.263", "module": "C2"}, {"value": "871.73", "module": "C3"}, {"value": "37.886", "module": "C4"}, {"value": "-14433", "module": "D"}]}, "resolvedFlowVersion": "38.00.000", "flowProperties": [], "typeOfFlow": "Other flow", "classification": {"classHierarchy": "Quantities", "name": "GaBiCategories"}}, {"dataSetInternalID": 5, "referenceToFlowDataSet": {"shortDescription": [{"value": "Non renewable primary energy as material utilization (PENRM)", "lang": "en"}, {"value": "Nicht-erneuerbare Primärenergie zur stofflichen Nutzung (PENRM)", "lang": "de"}], "type": "flow data set", "refObjectId": "1421caa0-679d-4bf4-b282-0eb850ccae27", "uri": "../flows/1421caa0-679d-4bf4-b282-0eb850ccae27.xml"}, "exchange direction": "INPUT", "other": {"anies": [{"name": "referenceToUnitGroupDataSet", "value": {"shortDescription": [{"value": "MJ", "lang": "en"}], "type": "unit group data set", "refObjectId": "93a60a57-a3c8-11da-a746-0800200c9a66", "uri": "../unitgroups/93a60a57-a3c8-11da-a746-0800200c9a66.xml"}}, {"value": "840.63", "module": "A1-A3"}, {"value": "0", "module": "A4"}, {"value": "0", "module": "A5"}, {"value": "0", "module": "B2"}, {"value": "0", "module": "B6"}, {"value": "0", "module": "C1"}, {"value": "0", "module": "C2"}, {"value": "-840.63", "module": "C3"}, {"value": "0", "module": "C4"}, {"value": "0", "module": "D"}]}, "resolvedFlowVersion": "38.00.000", "flowProperties": [], "typeOfFlow": "Other flow", "classification": {"classHierarchy": "Quantities", "name": "GaBiCategories"}}, {"dataSetInternalID": 6, "referenceToFlowDataSet": {"shortDescription": [{"value": "Total use of non renewable primary energy resources (PENRT)", "lang": "en"}, {"value": "Total nicht erneuerbare Primärenergie (PENRT)", "lang": "de"}], "type": "flow data set", "refObjectId": "06159210-646b-4c8d-8583-da9b3b95a6c1", "uri": "../flows/06159210-646b-4c8d-8583-da9b3b95a6c1.xml"}, "exchange direction": "INPUT", "other": {"anies": [{"name": "referenceToUnitGroupDataSet", "value": {"shortDescription": [{"value": "MJ", "lang": "en"}], "type": "unit group data set", "refObjectId": "93a60a57-a3c8-11da-a746-0800200c9a66", "uri": "../unitgroups/93a60a57-a3c8-11da-a746-0800200c9a66.xml"}}, {"value": "26979.51", "module": "A1-A3"}, {"value": "55.057", "module": "A4"}, {"value": "1.791", "module": "A5"}, {"value": "0", "module": "B2"}, {"value": "18545", "module": "B6"}, {"value": "0", "module": "C1"}, {"value": "27.263", "module": "C2"}, {"value": "31.095", "module": "C3"}, {"value": "37.886", "module": "C4"}, {"value": "-14433", "module": "D"}]}, "resolvedFlowVersion": "38.00.000", "flowProperties": [], "typeOfFlow": "Other flow", "classification": {"classHierarchy": "Quantities / Environmental quantities / EPD EN 15804 / LCI indicators", "name": "GaBiCategories"}}, {"dataSetInternalID": 7, "referenceToFlowDataSet": {"shortDescription": [{"value": "Use of secondary material (SM)", "lang": "en"}, {"value": "Einsatz von Sekundärstoffen (SM)", "lang": "de"}], "type": "flow data set", "refObjectId": "c6a1f35f-2d09-4f54-8dfb-97e502e1ce92", "uri": "../flows/c6a1f35f-2d09-4f54-8dfb-97e502e1ce92.xml"}, "exchange direction": "INPUT", "other": {"anies": [{"name": "referenceToUnitGroupDataSet", "value": {"shortDescription": [{"value": "kg", "lang": "en"}], "type": "unit group data set", "refObjectId": "ad38d542-3fe9-439d-9b95-2f5f7752acaf", "uri": "../unitgroups/ad38d542-3fe9-439d-9b95-2f5f7752acaf.xml"}}, {"value": "30.6", "module": "A1-A3"}, {"value": "0", "module": "A4"}, {"value": "0", "module": "A5"}, {"value": "0", "module": "B2"}, {"value": "0", "module": "B6"}, {"value": "0", "module": "C1"}, {"value": "0", "module": "C2"}, {"value": "0", "module": "C3"}, {"value": "0", "module": "C4"}, {"value": "0", "module": "D"}]}, "resolvedFlowVersion": "38.00.000", "flowProperties": [], "typeOfFlow": "Other flow", "classification": {"classHierarchy": "Quantities / Environmental quantities / EPD EN 15804 / LCI indicators", "name": "GaBiCategories"}}, {"dataSetInternalID": 8, "referenceToFlowDataSet": {"shortDescription": [{"value": "Use of renewable secondary fuels (RSF)", "lang": "en"}, {"value": "Erneuerbare Sekundärbrennstoffe (RSF)", "lang": "de"}], "type": "flow data set", "refObjectId": "64333088-a55f-4aa2-9a31-c10b07816787", "uri": "../flows/64333088-a55f-4aa2-9a31-c10b07816787.xml"}, "exchange direction": "INPUT", "other": {"anies": [{"name": "referenceToUnitGroupDataSet", "value": {"shortDescription": [{"value": "MJ", "lang": "en"}], "type": "unit group data set", "refObjectId": "93a60a57-a3c8-11da-a746-0800200c9a66", "uri": "../unitgroups/93a60a57-a3c8-11da-a746-0800200c9a66.xml"}}, {"value": "0", "module": "A1-A3"}, {"value": "0", "module": "A4"}, {"value": "0", "module": "A5"}, {"value": "0", "module": "B2"}, {"value": "0", "module": "B6"}, {"value": "0", "module": "C1"}, {"value": "0", "module": "C2"}, {"value": "0", "module": "C3"}, {"value": "0", "module": "C4"}, {"value": "0", "module": "D"}]}, "resolvedFlowVersion": "38.00.000", "flowProperties": [], "typeOfFlow": "Other flow", "classification": {"classHierarchy": "Quantities / Environmental quantities / EPD EN 15804 / LCI indicators", "name": "GaBiCategories"}}, {"dataSetInternalID": 9, "referenceToFlowDataSet": {"shortDescription": [{"value": "Use of non renewable secondary fuels (NRSF)", "lang": "en"}, {"value": "Nicht erneuerbare Sekundärbrennstoffe (NRSF)", "lang": "de"}], "type": "flow data set", "refObjectId": "89def144-d39a-4287-b86f-efde453ddcb2", "uri": "../flows/89def144-d39a-4287-b86f-efde453ddcb2.xml"}, "exchange direction": "INPUT", "other": {"anies": [{"name": "referenceToUnitGroupDataSet", "value": {"shortDescription": [{"value": "MJ", "lang": "en"}], "type": "unit group data set", "refObjectId": "93a60a57-a3c8-11da-a746-0800200c9a66", "uri": "../unitgroups/93a60a57-a3c8-11da-a746-0800200c9a66.xml"}}, {"value": "0", "module": "A1-A3"}, {"value": "0", "module": "A4"}, {"value": "0", "module": "A5"}, {"value": "0", "module": "B2"}, {"value": "0", "module": "B6"}, {"value": "0", "module": "C1"}, {"value": "0", "module": "C2"}, {"value": "0", "module": "C3"}, {"value": "0", "module": "C4"}, {"value": "0", "module": "D"}]}, "resolvedFlowVersion": "38.00.000", "flowProperties": [], "typeOfFlow": "Other flow", "classification": {"classHierarchy": "Quantities / Environmental quantities / EPD EN 15804 / LCI indicators", "name": "GaBiCategories"}}, {"dataSetInternalID": 10, "referenceToFlowDataSet": {"shortDescription": [{"value": "Use of net fresh water (FW)", "lang": "en"}, {"value": "Einsatz von Süßwasserressourcen (FW)", "lang": "de"}], "type": "flow data set", "refObjectId": "3cf952c8-f3a4-461d-8c96-96456ca62246", "uri": "../flows/3cf952c8-f3a4-461d-8c96-96456ca62246.xml"}, "exchange direction": "INPUT", "other": {"anies": [{"name": "referenceToUnitGroupDataSet", "value": {"shortDescription": [{"value": "m^3", "lang": "en"}], "type": "unit group data set", "refObjectId": "cd950537-0a98-4044-9ba7-9f9a68d0a504", "uri": "../unitgroups/cd950537-0a98-4044-9ba7-9f9a68d0a504.xml"}}, {"value": "20.6549189", "module": "A1-A3"}, {"value": "0.0003111", "module": "A4"}, {"value": "0.017", "module": "A5"}, {"value": "0", "module": "B2"}, {"value": "9.502", "module": "B6"}, {"value": "0", "module": "C1"}, {"value": "0.0001541", "module": "C2"}, {"value": "0.166", "module": "C3"}, {"value": "0.01", "module": "C4"}, {"value": "-11.421", "module": "D"}]}, "resolvedFlowVersion": "38.00.000", "flowProperties": [], "typeOfFlow": "Other flow", "classification": {"classHierarchy": "Quantities / Environmental quantities / EPD EN 15804 / LCI indicators", "name": "GaBiCategories"}}, {"dataSetInternalID": 11, "referenceToFlowDataSet": {"shortDescription": [{"value": "Hazardous waste disposed (HWD)", "lang": "en"}, {"value": "Gefährlicher Abfall zur Deponie (HWD)", "lang": "de"}], "type": "flow data set", "refObjectId": "430f9e0f-59b2-46a0-8e0d-55e0e84948fc", "uri": "../flows/430f9e0f-59b2-46a0-8e0d-55e0e84948fc.xml"}, "exchange direction": "OUTPUT", "other": {"anies": [{"name": "referenceToUnitGroupDataSet", "value": {"shortDescription": [{"value": "kg", "lang": "en"}], "type": "unit group data set", "refObjectId": "ad38d542-3fe9-439d-9b95-2f5f7752acaf", "uri": "../unitgroups/ad38d542-3fe9-439d-9b95-2f5f7752acaf.xml"}}, {"value": "6.366677E-05", "module": "A1-A3"}, {"value": "5.34E-09", "module": "A4"}, {"value": "2.639E-09", "module": "A5"}, {"value": "0", "module": "B2"}, {"value": "7.676E-06", "module": "B6"}, {"value": "0", "module": "C1"}, {"value": "2.644E-09", "module": "C2"}, {"value": "1.177E-07", "module": "C3"}, {"value": "5.774E-07", "module": "C4"}, {"value": "-0.0001295", "module": "D"}]}, "resolvedFlowVersion": "38.00.000", "flowProperties": [], "typeOfFlow": "Other flow", "classification": {"classHierarchy": "Quantities / Environmental quantities / EPD EN 15804 / LCI indicators", "name": "GaBiCategories"}}, {"dataSetInternalID": 12, "referenceToFlowDataSet": {"shortDescription": [{"value": "Non hazardous waste disposed (NHWD)", "lang": "en"}, {"value": "Entsorgter nicht gefährlicher Abfall (NHWD)", "lang": "de"}], "type": "flow data set", "refObjectId": "b29ef66b-e286-4afa-949f-62f1a7b4d7fa", "uri": "../flows/b29ef66b-e286-4afa-949f-62f1a7b4d7fa.xml"}, "exchange direction": "OUTPUT", "other": {"anies": [{"name": "referenceToUnitGroupDataSet", "value": {"shortDescription": [{"value": "kg", "lang": "en"}], "type": "unit group data set", "refObjectId": "ad38d542-3fe9-439d-9b95-2f5f7752acaf", "uri": "../unitgroups/ad38d542-3fe9-439d-9b95-2f5f7752acaf.xml"}}, {"value": "423.853", "module": "A1-A3"}, {"value": "0.006", "module": "A4"}, {"value": "0.178", "module": "A5"}, {"value": "0", "module": "B2"}, {"value": "13.156", "module": "B6"}, {"value": "0", "module": "C1"}, {"value": "0.003", "module": "C2"}, {"value": "6.916", "module": "C3"}, {"value": "190.46", "module": "C4"}, {"value": "-237.25", "module": "D"}]}, "resolvedFlowVersion": "38.00.000", "flowProperties": [], "typeOfFlow": "Other flow", "classification": {"classHierarchy": "Quantities / Environmental quantities / EPD EN 15804 / LCI indicators", "name": "GaBiCategories"}}, {"dataSetInternalID": 13, "referenceToFlowDataSet": {"shortDescription": [{"value": "Radioactive waste disposed (RWD)", "lang": "en"}, {"value": "Entsorgter radioaktiver Abfall (RWD)", "lang": "de"}], "type": "flow data set", "refObjectId": "3449546e-52ad-4b39-b809-9fb77cea8ff6", "uri": "../flows/3449546e-52ad-4b39-b809-9fb77cea8ff6.xml"}, "exchange direction": "OUTPUT", "other": {"anies": [{"name": "referenceToUnitGroupDataSet", "value": {"shortDescription": [{"value": "kg", "lang": "en"}], "type": "unit group data set", "refObjectId": "ad38d542-3fe9-439d-9b95-2f5f7752acaf", "uri": "../unitgroups/ad38d542-3fe9-439d-9b95-2f5f7752acaf.xml"}}, {"value": "1.2611745", "module": "A1-A3"}, {"value": "5.909E-05", "module": "A4"}, {"value": "9.411E-05", "module": "A5"}, {"value": "0", "module": "B2"}, {"value": "2.814", "module": "B6"}, {"value": "0", "module": "C1"}, {"value": "2.926E-05", "module": "C2"}, {"value": "0.001", "module": "C3"}, {"value": "0.0004311", "module": "C4"}, {"value": "-1.501", "module": "D"}]}, "resolvedFlowVersion": "38.00.000", "flowProperties": [], "typeOfFlow": "Other flow", "classification": {"classHierarchy": "Quantities / Environmental quantities / EPD EN 15804 / LCI indicators", "name": "GaBiCategories"}}, {"dataSetInternalID": 14, "referenceToFlowDataSet": {"shortDescription": [{"value": "Components for re-use (CRU)", "lang": "en"}, {"value": "Komponenten für die Wiederverwendung (CRU)", "lang": "de"}], "type": "flow data set", "refObjectId": "a2b32f97-3fc7-4af2-b209-525bc6426f33", "uri": "../flows/a2b32f97-3fc7-4af2-b209-525bc6426f33.xml"}, "exchange direction": "OUTPUT", "other": {"anies": [{"name": "referenceToUnitGroupDataSet", "value": {"shortDescription": [{"value": "kg", "lang": "en"}], "type": "unit group data set", "refObjectId": "ad38d542-3fe9-439d-9b95-2f5f7752acaf", "uri": "../unitgroups/ad38d542-3fe9-439d-9b95-2f5f7752acaf.xml"}}, {"value": "0", "module": "A1-A3"}, {"value": "0", "module": "A4"}, {"value": "0", "module": "A5"}, {"value": "0", "module": "B2"}, {"value": "0", "module": "B6"}, {"value": "0", "module": "C1"}, {"value": "0", "module": "C2"}, {"value": "0", "module": "C3"}, {"value": "0", "module": "C4"}, {"value": "0", "module": "D"}]}, "resolvedFlowVersion": "38.00.000", "flowProperties": [], "typeOfFlow": "Other flow", "classification": {"classHierarchy": "Quantities / Environmental quantities / EPD EN 15804 / LCI indicators", "name": "GaBiCategories"}}, {"dataSetInternalID": 15, "referenceToFlowDataSet": {"shortDescription": [{"value": "Materials for recycling (MFR)", "lang": "en"}, {"value": "Stoffe zum Recycling (MFR)", "lang": "de"}], "type": "flow data set", "refObjectId": "d7fe48a5-4103-49c8-9aae-b0b5dfdbd6ae", "uri": "../flows/d7fe48a5-4103-49c8-9aae-b0b5dfdbd6ae.xml"}, "exchange direction": "OUTPUT", "other": {"anies": [{"name": "referenceToUnitGroupDataSet", "value": {"shortDescription": [{"value": "kg", "lang": "en"}], "type": "unit group data set", "refObjectId": "ad38d542-3fe9-439d-9b95-2f5f7752acaf", "uri": "../unitgroups/ad38d542-3fe9-439d-9b95-2f5f7752acaf.xml"}}, {"value": "0", "module": "A1-A3"}, {"value": "0", "module": "A4"}, {"value": "0", "module": "A5"}, {"value": "0", "module": "B2"}, {"value": "0", "module": "B6"}, {"value": "0", "module": "C1"}, {"value": "0", "module": "C2"}, {"value": "242.36", "module": "C3"}, {"value": "0", "module": "C4"}, {"value": "0", "module": "D"}]}, "resolvedFlowVersion": "38.00.000", "flowProperties": [], "typeOfFlow": "Other flow", "classification": {"classHierarchy": "Quantities / Environmental quantities / EPD EN 15804 / LCI indicators", "name": "GaBiCategories"}}, {"dataSetInternalID": 16, "referenceToFlowDataSet": {"shortDescription": [{"value": "Materials for energy recovery (MER)", "lang": "en"}, {"value": "Stoffe für die Energierückgewinnung (MER)", "lang": "de"}], "type": "flow data set", "refObjectId": "59a9181c-3aaf-46ee-8b13-2b3723b6e447", "uri": "../flows/59a9181c-3aaf-46ee-8b13-2b3723b6e447.xml"}, "exchange direction": "OUTPUT", "other": {"anies": [{"name": "referenceToUnitGroupDataSet", "value": {"shortDescription": [{"value": "kg", "lang": "en"}], "type": "unit group data set", "refObjectId": "ad38d542-3fe9-439d-9b95-2f5f7752acaf", "uri": "../unitgroups/ad38d542-3fe9-439d-9b95-2f5f7752acaf.xml"}}, {"value": "0", "module": "A1-A3"}, {"value": "0", "module": "A4"}, {"value": "0", "module": "A5"}, {"value": "0", "module": "B2"}, {"value": "0", "module": "B6"}, {"value": "0", "module": "C1"}, {"value": "0", "module": "C2"}, {"value": "0", "module": "C3"}, {"value": "0", "module": "C4"}, {"value": "0", "module": "D"}]}, "resolvedFlowVersion": "38.00.000", "flowProperties": [], "typeOfFlow": "Other flow", "classification": {"classHierarchy": "Quantities / Environmental quantities / EPD EN 15804 / LCI indicators", "name": "GaBiCategories"}}, {"dataSetInternalID": 17, "referenceToFlowDataSet": {"shortDescription": [{"value": "Exported electrical energy (EEE)", "lang": "en"}, {"value": "Exportierte elektrische Energie (EEE)", "lang": "de"}], "type": "flow data set", "refObjectId": "4da0c987-2b76-40d6-9e9e-82a017aaaf29", "uri": "../flows/4da0c987-2b76-40d6-9e9e-82a017aaaf29.xml"}, "exchange direction": "OUTPUT", "other": {"anies": [{"name": "referenceToUnitGroupDataSet", "value": {"shortDescription": [{"value": "MJ", "lang": "en"}], "type": "unit group data set", "refObjectId": "93a60a57-a3c8-11da-a746-0800200c9a66", "uri": "../unitgroups/93a60a57-a3c8-11da-a746-0800200c9a66.xml"}}, {"value": "0", "module": "A1-A3"}, {"value": "0", "module": "A4"}, {"value": "8.58", "module": "A5"}, {"value": "0", "module": "B2"}, {"value": "0", "module": "B6"}, {"value": "0", "module": "C1"}, {"value": "0", "module": "C2"}, {"value": "0", "module": "C3"}, {"value": "0", "module": "C4"}, {"value": "0", "module": "D"}]}, "resolvedFlowVersion": "38.00.000", "flowProperties": [], "typeOfFlow": "Other flow", "classification": {"classHierarchy": "Quantities / Environmental quantities / EPD EN 15804 / LCI indicators", "name": "GaBiCategories"}}, {"dataSetInternalID": 18, "referenceToFlowDataSet": {"shortDescription": [{"value": "Exported thermal energy (EET)", "lang": "en"}, {"value": "Exportierte thermische Energie (EET)", "lang": "de"}], "type": "flow data set", "refObjectId": "98daf38a-7a79-46d3-9a37-2b7bd0955810", "uri": "../flows/98daf38a-7a79-46d3-9a37-2b7bd0955810.xml"}, "exchange direction": "OUTPUT", "other": {"anies": [{"name": "referenceToUnitGroupDataSet", "value": {"shortDescription": [{"value": "MJ", "lang": "en"}], "type": "unit group data set", "refObjectId": "93a60a57-a3c8-11da-a746-0800200c9a66", "uri": "../unitgroups/93a60a57-a3c8-11da-a746-0800200c9a66.xml"}}, {"value": "0", "module": "A1-A3"}, {"value": "0", "module": "A4"}, {"value": "15.561", "module": "A5"}, {"value": "0", "module": "B2"}, {"value": "0", "module": "B6"}, {"value": "0", "module": "C1"}, {"value": "0", "module": "C2"}, {"value": "0", "module": "C3"}, {"value": "0", "module": "C4"}, {"value": "0", "module": "D"}]}, "resolvedFlowVersion": "38.00.000", "flowProperties": [], "typeOfFlow": "Other flow", "classification": {"classHierarchy": "Quantities / Environmental quantities / EPD EN 15804 / LCI indicators", "name": "GaBiCategories"}}]}, "LCIAResults": {"LCIAResult": [{"referenceToLCIAMethodDataSet": {"shortDescription": [{"value": "Global Warming Potential total (GWP-total)", "lang": "en"}, {"value": "Globales Erwärmungspotenzial total (GWP-total)", "lang": "de"}], "type": "LCIA method data set", "refObjectId": "6a37f984-a4b3-458a-a20a-64418c145fa2", "uri": "../lciamethods/6a37f984-a4b3-458a-a20a-64418c145fa2.xml"}, "other": {"anies": [{"name": "referenceToUnitGroupDataSet", "value": {"shortDescription": [{"value": "kg CO_(2) eq", "lang": "en"}], "type": "unit group data set", "refObjectId": "1ebf3012-d0db-4de2-aefd-ef30cedb0be1", "uri": "../unitgroups/1ebf3012-d0db-4de2-aefd-ef30cedb0be1.xml"}}, {"value": "2042.23", "module": "A1-A3"}, {"value": "4.058", "module": "A4"}, {"value": "5.671", "module": "A5"}, {"value": "0", "module": "B2"}, {"value": "1059.7", "module": "B6"}, {"value": "0", "module": "C1"}, {"value": "2.01", "module": "C2"}, {"value": "67.721", "module": "C3"}, {"value": "2.904", "module": "C4"}, {"value": "-1048.4", "module": "D"}]}}, {"referenceToLCIAMethodDataSet": {"shortDescription": [{"value": "Global Warming Potential fossil fuels (GWP-fossil)", "lang": "en"}, {"value": "Globales Erwärmungspotenzial fossil (GWP-fossil)", "lang": "de"}], "type": "LCIA method data set", "refObjectId": "5f635281-343e-44fb-83df-1971b155e6b6", "uri": "../lciamethods/5f635281-343e-44fb-83df-1971b155e6b6.xml"}, "other": {"anies": [{"name": "referenceToUnitGroupDataSet", "value": {"shortDescription": [{"value": "kg CO_(2) eq", "lang": "en"}], "type": "unit group data set", "refObjectId": "1ebf3012-d0db-4de2-aefd-ef30cedb0be1", "uri": "../unitgroups/1ebf3012-d0db-4de2-aefd-ef30cedb0be1.xml"}}, {"value": "2046.761", "module": "A1-A3"}, {"value": "3.879", "module": "A4"}, {"value": "0.142", "module": "A5"}, {"value": "0", "module": "B2"}, {"value": "1054.7", "module": "B6"}, {"value": "0", "module": "C1"}, {"value": "1.921", "module": "C2"}, {"value": "66.525", "module": "C3"}, {"value": "2.886", "module": "C4"}, {"value": "-1045.2", "module": "D"}]}}, {"referenceToLCIAMethodDataSet": {"shortDescription": [{"value": "Global Warming Potential biogenic (GWP-biogenic)", "lang": "en"}, {"value": "Globales Erwärmungspotenzial biogen (GWP-biogenic)", "lang": "de"}], "type": "LCIA method data set", "refObjectId": "2356e1ab-0185-4db5-86e5-16de51c7485c", "uri": "../lciamethods/2356e1ab-0185-4db5-86e5-16de51c7485c.xml"}, "other": {"anies": [{"name": "referenceToUnitGroupDataSet", "value": {"shortDescription": [{"value": "kg CO_(2) eq", "lang": "en"}], "type": "unit group data set", "refObjectId": "1ebf3012-d0db-4de2-aefd-ef30cedb0be1", "uri": "../unitgroups/1ebf3012-d0db-4de2-aefd-ef30cedb0be1.xml"}}, {"value": "-5.496", "module": "A1-A3"}, {"value": "0.179", "module": "A4"}, {"value": "5.529", "module": "A5"}, {"value": "0", "module": "B2"}, {"value": "3.516", "module": "B6"}, {"value": "0", "module": "C1"}, {"value": "0.089", "module": "C2"}, {"value": "1.192", "module": "C3"}, {"value": "0.01", "module": "C4"}, {"value": "-2.993", "module": "D"}]}}, {"referenceToLCIAMethodDataSet": {"shortDescription": [{"value": "Global Warming Potential luluc (GWP-luluc)", "lang": "en"}, {"value": "Globales Erwärmungspotenzial luluc (GWP-luluc)", "lang": "de"}], "type": "LCIA method data set", "refObjectId": "4331bbdb-978a-490d-8707-eeb047f01a55", "uri": "../lciamethods/4331bbdb-978a-490d-8707-eeb047f01a55.xml"}, "other": {"anies": [{"name": "referenceToUnitGroupDataSet", "value": {"shortDescription": [{"value": "kg CO_(2) eq", "lang": "en"}], "type": "unit group data set", "refObjectId": "1ebf3012-d0db-4de2-aefd-ef30cedb0be1", "uri": "../unitgroups/1ebf3012-d0db-4de2-aefd-ef30cedb0be1.xml"}}, {"value": "0.9722727", "module": "A1-A3"}, {"value": "9.231E-05", "module": "A4"}, {"value": "9.331E-05", "module": "A5"}, {"value": "0", "module": "B2"}, {"value": "1.529", "module": "B6"}, {"value": "0", "module": "C1"}, {"value": "4.571E-05", "module": "C2"}, {"value": "0.004", "module": "C3"}, {"value": "0.008", "module": "C4"}, {"value": "-0.194", "module": "D"}]}}, {"referenceToLCIAMethodDataSet": {"shortDescription": [{"value": "Depletion potential of the stratospheric ozone layer (ODP)", "lang": "en"}, {"value": "Abbau Potential der stratosphärischen Ozonschicht (ODP)", "lang": "de"}], "type": "LCIA method data set", "refObjectId": "b5c629d6-def3-11e6-bf01-fe55135034f3", "uri": "../lciamethods/b5c629d6-def3-11e6-bf01-fe55135034f3.xml"}, "other": {"anies": [{"name": "referenceToUnitGroupDataSet", "value": {"shortDescription": [{"value": "kg CFC11 eq", "lang": "en"}], "type": "unit group data set", "refObjectId": "d9e957c9-7309-4474-bf3a-7777df6c4e5b", "uri": "../unitgroups/d9e957c9-7309-4474-bf3a-7777df6c4e5b.xml"}}, {"value": "6.477621209E-09", "module": "A1-A3"}, {"value": "4.095E-16", "module": "A4"}, {"value": "1.022E-15", "module": "A5"}, {"value": "0", "module": "B2"}, {"value": "2.32E-11", "module": "B6"}, {"value": "0", "module": "C1"}, {"value": "2.028E-16", "module": "C2"}, {"value": "3.369E-14", "module": "C3"}, {"value": "1.07E-14", "module": "C4"}, {"value": "-7.33E-09", "module": "D"}]}}, {"referenceToLCIAMethodDataSet": {"shortDescription": [{"value": "Acidification potential of land and water (AP)", "lang": "en"}, {"value": "Versauerungspotenzial von Boden und Wasser (AP)", "lang": "de"}], "type": "LCIA method data set", "refObjectId": "b5c611c6-def3-11e6-bf01-fe55135034f3", "uri": "../lciamethods/b5c611c6-def3-11e6-bf01-fe55135034f3.xml"}, "other": {"anies": [{"name": "referenceToUnitGroupDataSet", "value": {"shortDescription": [{"value": "mol H^(+) eq", "lang": "en"}], "type": "unit group data set", "refObjectId": "42e089ac-92bf-4bf2-8ca1-5fc40d18f2ed", "uri": "../unitgroups/42e089ac-92bf-4bf2-8ca1-5fc40d18f2ed.xml"}}, {"value": "10.224", "module": "A1-A3"}, {"value": "0.004", "module": "A4"}, {"value": "0.002", "module": "A5"}, {"value": "0", "module": "B2"}, {"value": "2.328", "module": "B6"}, {"value": "0", "module": "C1"}, {"value": "0.002", "module": "C2"}, {"value": "0.012", "module": "C3"}, {"value": "0.021", "module": "C4"}, {"value": "-3.891", "module": "D"}]}}, {"referenceToLCIAMethodDataSet": {"shortDescription": [{"value": "Eutrophication potential aquatic freshwater (EP-freshwater)", "lang": "en"}, {"value": "Eutrophierungspotenzial Süßwasser (EP-freshwater)", "lang": "de"}], "type": "LCIA method data set", "refObjectId": "b53ec18f-7377-4ad3-86eb-cc3f4f276b2b", "uri": "../lciamethods/b53ec18f-7377-4ad3-86eb-cc3f4f276b2b.xml"}, "other": {"anies": [{"name": "referenceToUnitGroupDataSet", "value": {"shortDescription": [{"value": "kg P eq", "lang": "en"}], "type": "unit group data set", "refObjectId": "0429039d-a61d-4590-ba67-aa4a20a810a1", "uri": "../unitgroups/0429039d-a61d-4590-ba67-aa4a20a810a1.xml"}}, {"value": "0.002213952", "module": "A1-A3"}, {"value": "8.301E-07", "module": "A4"}, {"value": "1.999E-07", "module": "A5"}, {"value": "0", "module": "B2"}, {"value": "0.003", "module": "B6"}, {"value": "0", "module": "C1"}, {"value": "4.111E-07", "module": "C2"}, {"value": "5.371E-06", "module": "C3"}, {"value": "4.957E-06", "module": "C4"}, {"value": "-0.0005496", "module": "D"}]}}, {"referenceToLCIAMethodDataSet": {"shortDescription": [{"value": "Eutrophication potential aquatic marine (EP-marine)", "lang": "en"}, {"value": "Eutrophierungspotenzial Salzwasser (EP-marine)", "lang": "de"}], "type": "LCIA method data set", "refObjectId": "b5c619fa-def3-11e6-bf01-fe55135034f3", "uri": "../lciamethods/b5c619fa-def3-11e6-bf01-fe55135034f3.xml"}, "other": {"anies": [{"name": "referenceToUnitGroupDataSet", "value": {"shortDescription": [{"value": "kg N eq", "lang": "en"}], "type": "unit group data set", "refObjectId": "d05bb823-ecdf-4686-8c40-bf1d9257859f", "uri": "../unitgroups/d05bb823-ecdf-4686-8c40-bf1d9257859f.xml"}}, {"value": "1.637", "module": "A1-A3"}, {"value": "0.001", "module": "A4"}, {"value": "0.0005735", "module": "A5"}, {"value": "0", "module": "B2"}, {"value": "0.517", "module": "B6"}, {"value": "0", "module": "C1"}, {"value": "0.0006117", "module": "C2"}, {"value": "0.003", "module": "C3"}, {"value": "0.005", "module": "C4"}, {"value": "-0.515", "module": "D"}]}}, {"referenceToLCIAMethodDataSet": {"shortDescription": [{"value": "Eutrophication potential terrestrial (EP-terrestrial)", "lang": "en"}, {"value": "Eutrophierungspotenzial Land (EP-terrestrial)", "lang": "de"}], "type": "LCIA method data set", "refObjectId": "b5c614d2-def3-11e6-bf01-fe55135034f3", "uri": "../lciamethods/b5c614d2-def3-11e6-bf01-fe55135034f3.xml"}, "other": {"anies": [{"name": "referenceToUnitGroupDataSet", "value": {"shortDescription": [{"value": "mol N eq", "lang": "en"}], "type": "unit group data set", "refObjectId": "71b4d617-0ec9-4d3f-b65e-e438940c2401", "uri": "../unitgroups/71b4d617-0ec9-4d3f-b65e-e438940c2401.xml"}}, {"value": "18.079", "module": "A1-A3"}, {"value": "0.014", "module": "A4"}, {"value": "0.007", "module": "A5"}, {"value": "0", "module": "B2"}, {"value": "5.434", "module": "B6"}, {"value": "0", "module": "C1"}, {"value": "0.007", "module": "C2"}, {"value": "0.055", "module": "C3"}, {"value": "0.059", "module": "C4"}, {"value": "-5.557", "module": "D"}]}}, {"referenceToLCIAMethodDataSet": {"shortDescription": [{"value": "Formation potential of tropospheric ozone photochemical oxidants (POCP)", "lang": "en"}, {"value": "Bildungspotential für troposphärisches Ozon (POCP)", "lang": "de"}], "type": "LCIA method data set", "refObjectId": "b5c610fe-def3-11e6-bf01-fe55135034f3", "uri": "../lciamethods/b5c610fe-def3-11e6-bf01-fe55135034f3.xml"}, "other": {"anies": [{"name": "referenceToUnitGroupDataSet", "value": {"shortDescription": [{"value": "kg NMVOC eq", "lang": "en"}], "type": "unit group data set", "refObjectId": "d27c25f8-fbc1-44c6-b47b-4adbae4199c6", "uri": "../unitgroups/d27c25f8-fbc1-44c6-b47b-4adbae4199c6.xml"}}, {"value": "4.56", "module": "A1-A3"}, {"value": "0.003", "module": "A4"}, {"value": "0.002", "module": "A5"}, {"value": "0", "module": "B2"}, {"value": "1.417", "module": "B6"}, {"value": "0", "module": "C1"}, {"value": "0.002", "module": "C2"}, {"value": "0.008", "module": "C3"}, {"value": "0.016", "module": "C4"}, {"value": "-1.663", "module": "D"}]}}, {"referenceToLCIAMethodDataSet": {"shortDescription": [{"value": "Abiotic depletion potential for non fossil resources (ADPE)", "lang": "en"}, {"value": "Potenzial für den abiotischen Abbau nicht fossiler Ressourcen (ADPE)", "lang": "de"}], "type": "LCIA method data set", "refObjectId": "b2ad6494-c78d-11e6-9d9d-cec0c932ce01", "uri": "../lciamethods/b2ad6494-c78d-11e6-9d9d-cec0c932ce01.xml"}, "other": {"anies": [{"name": "referenceToUnitGroupDataSet", "value": {"shortDescription": [{"value": "kg Sb eq", "lang": "en"}], "type": "unit group data set", "refObjectId": "54ccd2d9-a32a-4fc2-923d-f2c8c93e89d4", "uri": "../unitgroups/54ccd2d9-a32a-4fc2-923d-f2c8c93e89d4.xml"}}, {"value": "0.0270003436", "module": "A1-A3"}, {"value": "1.163E-07", "module": "A4"}, {"value": "1.614E-08", "module": "A5"}, {"value": "0", "module": "B2"}, {"value": "0.0003053", "module": "B6"}, {"value": "0", "module": "C1"}, {"value": "5.76E-08", "module": "C2"}, {"value": "4.623E-07", "module": "C3"}, {"value": "2.592E-07", "module": "C4"}, {"value": "-0.009", "module": "D"}]}}, {"referenceToLCIAMethodDataSet": {"shortDescription": [{"value": "Abiotic depletion potential for fossil resources (ADPF)", "lang": "en"}, {"value": "Potenzial für den abiotischen Abbau fossiler Brennstoffe (ADPF)", "lang": "de"}], "type": "LCIA method data set", "refObjectId": "b2ad6110-c78d-11e6-9d9d-cec0c932ce01", "uri": "../lciamethods/b2ad6110-c78d-11e6-9d9d-cec0c932ce01.xml"}, "other": {"anies": [{"name": "referenceToUnitGroupDataSet", "value": {"shortDescription": [{"value": "MJ", "lang": "en"}], "type": "unit group data set", "refObjectId": "93a60a57-a3c8-11da-a746-0800200c9a66", "uri": "../unitgroups/93a60a57-a3c8-11da-a746-0800200c9a66.xml"}}, {"value": "26960.25", "module": "A1-A3"}, {"value": "55.003", "module": "A4"}, {"value": "1.79", "module": "A5"}, {"value": "0", "module": "B2"}, {"value": "18541", "module": "B6"}, {"value": "0", "module": "C1"}, {"value": "27.237", "module": "C2"}, {"value": "31.087", "module": "C3"}, {"value": "37.868", "module": "C4"}, {"value": "-14428", "module": "D"}]}}, {"referenceToLCIAMethodDataSet": {"shortDescription": [{"value": "Water use (WDP)", "lang": "en"}, {"value": "Wassernutzung (WDP)", "lang": "de"}], "type": "LCIA method data set", "refObjectId": "b2ad66ce-c78d-11e6-9d9d-cec0c932ce01", "uri": "../lciamethods/b2ad66ce-c78d-11e6-9d9d-cec0c932ce01.xml"}, "other": {"anies": [{"name": "referenceToUnitGroupDataSet", "value": {"shortDescription": [{"value": "m^(3) world eq deprived", "lang": "en"}], "type": "unit group data set", "refObjectId": "6ae2df01-888e-46c8-b17d-49fa3869b476", "uri": "../unitgroups/6ae2df01-888e-46c8-b17d-49fa3869b476.xml"}}, {"value": "248.178", "module": "A1-A3"}, {"value": "0.008", "module": "A4"}, {"value": "0.703", "module": "A5"}, {"value": "0", "module": "B2"}, {"value": "229.89", "module": "B6"}, {"value": "0", "module": "C1"}, {"value": "0.004", "module": "C2"}, {"value": "6.926", "module": "C3"}, {"value": "0.303", "module": "C4"}, {"value": "-60.15", "module": "D"}]}}, {"referenceToLCIAMethodDataSet": {"shortDescription": [{"value": "Incidence of disease due to PM emissions (PM)", "lang": "en"}, {"value": "Auftreten von Krankheiten aufgrund von Feinstaubemissionen (PM)", "lang": "de"}], "type": "LCIA method data set", "refObjectId": "b5c602c6-def3-11e6-bf01-fe55135034f3", "uri": "../lciamethods/b5c602c6-def3-11e6-bf01-fe55135034f3.xml"}, "other": {"anies": [{"name": "referenceToUnitGroupDataSet", "value": {"shortDescription": [{"value": "Disease incidence", "lang": "en"}], "type": "unit group data set", "refObjectId": "3883559b-648f-4afc-8ba2-0bd24f3affa3", "uri": "../unitgroups/3883559b-648f-4afc-8ba2-0bd24f3affa3.xml"}}, {"value": "9.695508E-05", "module": "A1-A3"}, {"value": "2.041E-08", "module": "A4"}, {"value": "8.798E-09", "module": "A5"}, {"value": "0", "module": "B2"}, {"value": "1.953E-05", "module": "B6"}, {"value": "0", "module": "C1"}, {"value": "1.011E-08", "module": "C2"}, {"value": "1.519E-07", "module": "C3"}, {"value": "2.563E-07", "module": "C4"}, {"value": "-6.174E-05", "module": "D"}]}}, {"referenceToLCIAMethodDataSet": {"shortDescription": [{"value": "Human exposure efficiency relative to U235 (IR)", "lang": "en"}, {"value": "Wirkung durch Exposition des Menschen mit U235 (IR)", "lang": "de"}], "type": "LCIA method data set", "refObjectId": "b5c632be-def3-11e6-bf01-fe55135034f3", "uri": "../lciamethods/b5c632be-def3-11e6-bf01-fe55135034f3.xml"}, "other": {"anies": [{"name": "referenceToUnitGroupDataSet", "value": {"shortDescription": [{"value": "kBq U235 eq", "lang": "en"}], "type": "unit group data set", "refObjectId": "456b05bf-1415-44a9-9993-02452f554c09", "uri": "../unitgroups/456b05bf-1415-44a9-9993-02452f554c09.xml"}}, {"value": "242.244", "module": "A1-A3"}, {"value": "0.008", "module": "A4"}, {"value": "0.015", "module": "A5"}, {"value": "0", "module": "B2"}, {"value": "461.67", "module": "B6"}, {"value": "0", "module": "C1"}, {"value": "0.004", "module": "C2"}, {"value": "0.105", "module": "C3"}, {"value": "0.044", "module": "C4"}, {"value": "-301.19", "module": "D"}]}}, {"referenceToLCIAMethodDataSet": {"shortDescription": [{"value": "Comparative toxic unit for ecosystems (ETP-fw)", "lang": "en"}, {"value": "Toxizitätsvergleichseinheit für Ökosysteme (ETP-fw)", "lang": "de"}], "type": "LCIA method data set", "refObjectId": "ee1082d1-b0f7-43ca-a1f0-21e2a4a74511", "uri": "../lciamethods/ee1082d1-b0f7-43ca-a1f0-21e2a4a74511.xml"}, "other": {"anies": [{"name": "referenceToUnitGroupDataSet", "value": {"shortDescription": [{"value": "CTUe", "lang": "en"}], "type": "unit group data set", "refObjectId": "aa959ded-f1eb-4efb-9c5c-2d60be36b3e6", "uri": "../unitgroups/aa959ded-f1eb-4efb-9c5c-2d60be36b3e6.xml"}}, {"value": "14186.33", "module": "A1-A3"}, {"value": "38.99", "module": "A4"}, {"value": "0.85", "module": "A5"}, {"value": "0", "module": "B2"}, {"value": "7931.4", "module": "B6"}, {"value": "0", "module": "C1"}, {"value": "19.307", "module": "C2"}, {"value": "11.684", "module": "C3"}, {"value": "21.636", "module": "C4"}, {"value": "-5142.3", "module": "D"}]}}, {"referenceToLCIAMethodDataSet": {"shortDescription": [{"value": "Comparative toxic unit for humans (carcinogenic) (HTP-c)", "lang": "en"}, {"value": "Toxizitätsvergleichseinheit für Menschen (krebserregend) (HTP-c)", "lang": "de"}], "type": "LCIA method data set", "refObjectId": "2299222a-bbd8-474f-9d4f-4dd1f18aea7c", "uri": "../lciamethods/2299222a-bbd8-474f-9d4f-4dd1f18aea7c.xml"}, "other": {"anies": [{"name": "referenceToUnitGroupDataSet", "value": {"shortDescription": [{"value": "CTUh", "lang": "en"}], "type": "unit group data set", "refObjectId": "d4c9523e-2d7e-49fd-8469-998f547d3a70", "uri": "../unitgroups/d4c9523e-2d7e-49fd-8469-998f547d3a70.xml"}}, {"value": "8.508306E-06", "module": "A1-A3"}, {"value": "7.334E-10", "module": "A4"}, {"value": "4.494E-11", "module": "A5"}, {"value": "0", "module": "B2"}, {"value": "2.191E-07", "module": "B6"}, {"value": "0", "module": "C1"}, {"value": "3.632E-10", "module": "C2"}, {"value": "1.009E-09", "module": "C3"}, {"value": "3.206E-09", "module": "C4"}, {"value": "-2.48E-07", "module": "D"}]}}, {"referenceToLCIAMethodDataSet": {"shortDescription": [{"value": "Comparative toxic unit for humans (noncarcinogenic) (HTP-nc)", "lang": "en"}, {"value": "Toxizitätsvergleichseinheit für Menschen (nicht krebserregend) (HTP-nc)", "lang": "de"}], "type": "LCIA method data set", "refObjectId": "3af763a5-b7a1-48c9-9cee-1f223481fcef", "uri": "../lciamethods/3af763a5-b7a1-48c9-9cee-1f223481fcef.xml"}, "other": {"anies": [{"name": "referenceToUnitGroupDataSet", "value": {"shortDescription": [{"value": "CTUh", "lang": "en"}], "type": "unit group data set", "refObjectId": "d4c9523e-2d7e-49fd-8469-998f547d3a70", "uri": "../unitgroups/d4c9523e-2d7e-49fd-8469-998f547d3a70.xml"}}, {"value": "2.586589E-05", "module": "A1-A3"}, {"value": "3.136E-08", "module": "A4"}, {"value": "1.947E-09", "module": "A5"}, {"value": "0", "module": "B2"}, {"value": "8.071E-06", "module": "B6"}, {"value": "0", "module": "C1"}, {"value": "1.553E-08", "module": "C2"}, {"value": "1.017E-07", "module": "C3"}, {"value": "3.534E-07", "module": "C4"}, {"value": "-8.194E-06", "module": "D"}]}}, {"referenceToLCIAMethodDataSet": {"shortDescription": [{"value": "Soil quality index (SQP)", "lang": "en"}, {"value": "Bodenqualitätsindex (SQP)", "lang": "de"}], "type": "LCIA method data set", "refObjectId": "b2ad6890-c78d-11e6-9d9d-cec0c932ce01", "uri": "../lciamethods/b2ad6890-c78d-11e6-9d9d-cec0c932ce01.xml"}, "other": {"anies": [{"name": "referenceToUnitGroupDataSet", "value": {"shortDescription": [{"value": "SQP", "lang": "en"}], "type": "unit group data set", "refObjectId": "f130951c-e67f-4f7f-8dd4-665de3974e18", "uri": "../unitgroups/f130951c-e67f-4f7f-8dd4-665de3974e18.xml"}}, {"value": "3062.958", "module": "A1-A3"}, {"value": "0.141", "module": "A4"}, {"value": "0.475", "module": "A5"}, {"value": "0", "module": "B2"}, {"value": "5905.2", "module": "B6"}, {"value": "0", "module": "C1"}, {"value": "0.07", "module": "C2"}, {"value": "9.305", "module": "C3"}, {"value": "7.895", "module": "C4"}, {"value": "-492.86", "module": "D"}]}}]}, "otherAttributes": {"{http://www.indata.network/EPD/2019}epd-version": "1.2"}, "version": "1.1", "locations": "../ILCDLocations.xml"}