{"processInformation": {"dataSetInformation": {"UUID": "f5a00a9b-7d3f-440a-8c18-21c6f10a4976", "name": {"baseName": [{"value": "AWADUKT nevoPP SN10", "lang": "de"}, {"value": "AWADUKT nevoPP SN10", "lang": "en"}], "functionalUnitFlowProperties": [{"lang": "de"}]}, "classificationInformation": {"classification": [{"class": [{"value": "Kunststoffe", "level": 0, "classId": "6"}, {"value": "Rohre", "level": 1, "classId": "6.1"}, {"value": "Abwasserrohre", "level": 2, "classId": "6.1.02"}], "name": "OEKOBAU.DAT"}, {"class": [{"value": "03 Gebäudetechnik", "level": 0}, {"value": "Anlagen zur Wasserversorgung und -entsorgung", "level": 1}, {"value": "Drucklose Abwasserrohrsysteme aus Kunststoff", "level": 2}], "name": "IBUCategories"}]}, "generalComment": [{"value": "Die EPD gilt fr das Kanalrohrsystem AWADUKT nevoPP SN10. \nDas System besteht aus glatten Rohren und aufgesetzten Formteilen mit Dichtring als Verbindungsstcke. Die Kernschicht der Rohre besteht aus Polypropylen (PP) aus Post-Industrial-Rezyklat (PIR). Die Schichten an der Innen- und Auenseite des Rohrs sind aus fllstofffreiem PP aus Neuware hergestellt, ebenso wie die kompletten Formteile.\n\nDie Herstellung der Kanalrohrsysteme erfolgt in Deutschland. Die Produkte werden weltweit verwendet, mit einem Fokus auf Europa.", "lang": "de"}, {"value": "This EPD covers the sewage pipe system AWADUKT nevoPP SN10. \nThe system consists of smooth piping and moulded parts fitted to it with sealing ring acting as connectors. The core layer of the piping consists of polypropylene (PP) derived from post-industrial recyclate (PIR). The layers of the inner and outer side of the piping and the moulded parts are made from filler-free, new PP material. \n\nThe sewage pipe systems are manufactured in Germany. The products are used worldwide, with particular focus on Europe.", "lang": "en"}], "referenceToExternalDocumentation": [{"shortDescription": [{"value": "Anhang_Massebezug_AWADUKT_nevoPP.pdf (Massenbezüge AWADUKT nevoPP)", "lang": "de"}], "type": "source data set", "refObjectId": "ee575c1b-893c-4bfe-950e-c4c81e6eeb39"}], "other": {"anies": [{"scenario": [{"description": [{"value": "100% Recycling (C3/1, D/1)", "lang": "de"}, {"value": "100% Recycling (C3/1, D/1)", "lang": "en"}], "name": "S1", "default": true}, {"description": [{"value": "100% Verbrennung mit Energierückgewinnung(C3/2, D/2)", "lang": "de"}, {"value": "100% Combustion with energy recovery (C3/2, D/2)", "lang": "en"}], "name": "S2"}, {"description": [{"value": "100% Deponierung (C4/3, D/3)", "lang": "de"}, {"value": "100% Landfilling (C4/3, D/3)", "lang": "en"}], "name": "S3"}]}]}}, "quantitativeReference": {"referenceToReferenceFlow": [0]}, "time": {"referenceYear": 2024, "dataSetValidUntil": 2029, "other": {"anies": [{"name": "publicationDateOfEPD", "value": 1720396800000}]}}, "geography": {"locationOfOperationSupplyOrProduction": {"location": "DE"}}, "technology": {"technologyDescriptionAndIncludedProcesses": [{"value": "Bei dem deklarierten Produkt AWADUKT nevoPP SN10 handelt es sich um ein Kanalrohrsystem für den Tiefbau. Das Rohrsystem besteht aus Rohrprofilen, Formteilen als Verbindungselemente und Dichtringen zur Abdichtung des Systems. Bei den Rohrprofilen besteht die Kernschicht aus Polypropylen (PP) aus Post-Industrial-Rezyklat, die Außen- und Innenschicht aus füllstofffreier PP-Neuware. Die Rohrprofile werden dabei im Extrusionsverfahren hergestellt, die Formteile dagegen per Spritzguss. \nTechnische Daten: \nDie technischen Daten der Produkte, die im Geltungsbereich der EPD liegen, sind unter Verweis auf die den einzelnen Daten zugrundeliegenden Prfregeln genannt.\nDie Leistungswerte des Produkts in Bezug auf dessen Merkmale gelten nach den magebenden technischen Bestimmungen (einschlgige EN-Rohrnormen). \nDeklarierte Einheit: \nAls deklarierte Einheit wird \"1 kg Rohrsystem ohne Produktverpackung\" verwendet, das die Komponenten Rohr, Formteil und Dichtungsring umfasst. Eine massenanteilige Aufteilung der Komponenten ist in 2.5 dargestellt. Die Produktverpackung wird separat zum Produkt betrachtet und ebenfalls in die kobilanz miteinbezogen.\n\nFr die LCA wurde eine Durchschnittsvariante ber die Nennweiten des Rohrsystems AWADUKT nevoPP SN10 bilanziert. Der Massebezug unterscheidet sich je nach Nennweite des Rohres. Die Massebezge fr alle Varianten sind im Anhang zu finden.", "lang": "de"}, {"value": "The declared product AWADUKT nevoPP SN10 is a sewer pipe system for civil engineering. The pipe system consists of pipe profiles, fittings as connecting elements and sealing rings to seal the system. The core layer of the pipe profiles is made of polypropylene (PP) from post-industrial recyclate, while the outer and inner layers are made of filler-free virgin PP. The pipe profiles are produced by extrusion, while the molded parts are injection-molded. \nTechnical data: \nThe technical data of the products covered by this EPD are given with reference to the assessment rules underlying the individual data. \nThe products performance data with respect to its properties apply under the relevant technical regulations (relevant EN piping standards). \nDeclared unit: \nThe declared unit is 1 kg pipe system without product packaging, encompassing the components piping, moulded part, and sealing ring. 2.5 shows the mass fractions of the single components. The product packaging is considered separately from the product and is also included in the life-cycle assessment. \n\nAn average variant across the nominal widths of the AWADUKT nevoPP pipe system was assessed for the LCA. The mass relation varies subject to the pipes nominal width. The mass relations of all variants are given in the appendix.", "lang": "en"}], "technologicalApplicability": [{"value": "Das Rohrsystem AWADUKT nevoPP wird fr Kanle im Tiefbau eingesetzt. Das Rohrsystem wird angewandt zur Leitung von Abwssern, Regenwasser und Schmutz- und Mischwssern. Besonders geeignet ist die Variante fr die Haus- und Grundstcksentwsserung.", "lang": "de"}, {"value": "The AWADUKT nevoPP pipe system is used for sewer lines in underground engineering. The pipe system is used to rout wastewater, rain water, sewage, and mixed water. The variant is particularly suited for draining buildings and properties.", "lang": "en"}]}}, "modellingAndValidation": {"LCIMethodAndAllocation": {"typeOfDataSet": "EPD", "referenceToLCAMethodDetails": [{"shortDescription": [{"value": "Drucklose Abwasserrohrsysteme aus Kunststoff.pdf", "lang": "de"}], "type": "source data set", "refObjectId": "f3ba6276-217f-437e-9c62-05873d3fde0a"}], "other": {"anies": [{"name": "subType", "value": "average dataset"}]}}, "dataSourcesTreatmentAndRepresentativeness": {"referenceToDataSource": [{"shortDescription": [{"value": "GaBi Database (all versions)", "lang": "de"}], "type": "source data set", "refObjectId": "28d74cc0-db8b-4d7e-bc44-5f6d56ce0c4a"}, {"shortDescription": [{"value": "Sphera MLC (fka GaBi) CUP 2023.01", "lang": "de"}], "type": "source data set", "refObjectId": "6bcd5bfa-3623-48ab-a52b-6d5be8db82ed"}], "useAdviceForDataSet": [{"value": "Gültigkeitsbereich: \nDie EPD gilt fr das Kanalrohrsystem\nAWADUKT nevoPP SN10\nhergestellt im\nREHAU-Werk Viechtach, Deutschlandder Firma\n\nREHAU Industries SE & Co. KG.\n\nEs handelt sich um eine Durchschnitts-EPD, basierend auf einer durchschnittlichen Produktvariante, welche die Rohrsysteme verschiedener Nennweiten abdeckt. Die Bilanzierung erfolgt ber einen reprsentativen Produktionszeitraum. \nSystemgrenze: \nEs wird der gesamte Produktlebenszyklus von AWADUKT nevoPP betrachtet - siehe Flieschema.\nTyp der EPD: Wiege bis Bahre (Module A, B, C, D).\n\nDas nachfolgende Flieschema zeigt die Systemgrenzen bei der Bilanzierung von AWADUKT nevoPP:\n\nIm Folgenden sind die bercksichtigten Lebenswegabschnitte bzw. Prozessmodule fr die Herstellung der Rohrsysteme detailliert aufgelistet:\n\nA1 – A3 Herstellungsphase\nProduktion der Roh-, Hilfs- und Betriebsstoffe sowie der Vorprodukte inkl. Transport zum jeweiligen Werk\nRegranulierung des Rezyklats aus Mahlgut inkl. Transport nach Viechtach\nEnergiebereitstellung fr die Produktion\nProduktion und Verpackung des Rohrsystems im Werk Viechtach\nInterne Wiederaufbereitung der Produktionsabflle und Rckfhrung in Produktion\n\nVerwertung weiterer Abflle inkl. Transport\nA4 - A5 Aufbauphase\nTransport des Produkts zur Baustelle\nEinbau des Rohrsystems\nVerwertung der Produktverpackung\n\nB Nutzungsphase\nNutzung des Rohrsystems (B1)\nInstandhaltung des Rohrsystems (B2)\n\nC1 – C4 Entsorgung\nEs werden drei 100%-Entsorgungsszenarien angenommen:\nEnd-of-Life (EoL) Szenario 1: 100% Rckbau des Rohrsystems mit anschlieender werkstofflicher Verwertung (Modul C3/1 und D/1).\nEoL-Szenario 2: 100% Rckbau des Rohrsystems mit anschlieender energetischer Verwertung (Modul C3/2 und D/2).\nEoL-Szenario 3: 100% Rckbau des Rohrsystems und Entsorgung auf einer lokalen Deponie (Modul C4/3 und D/3)\n\nD Wiederverwendungs-, Rckgewinnungs- und/oder Recyclingpotentiale\nWiederverwendungs-, Rckgewinnungs-, und/oder Recyclingpotentiale sind in den Entsorgungsszenarien vorhanden, da hier die Rohrsysteme einer energetischen bzw. stofflichen Verwertung zugefhrt werden, aus denen Energie bzw. Sekundrmaterialien zurckgewonnen werden, die auerhalb der Systemgrenze genutzt werden knnen.", "lang": "de"}, {"value": "Scope: \nThis EPD covers the sewage pipe system \n\nAWADUKT nevoPP SN10manufactured at\nREHAU plant Viechtach, Germany, of the company\nREHAU Industries SE & Co. KG. \n\nThis is an average EPD based on an average product variant which covers the pipe systems with different nominal widths. The life-cycle assessment is performed over a representative production period. \nSystem boundary: \nThe entire product life cycle of AWADUKT nevoPP is considered, see the flow diagram. \nEPD type: cradle to the grave (modules A, B, C, and D). \n\nThe following flow diagram shows the system boundaries in the life-cycle assessment of AWADUKT nevoPP:\n\n\nThe life cycle segments or process modules for the manufacture of the pipe systems are detailed below. \n\nA1 – A3 Manufacturing phase \n\nProduction of the base, auxiliary and operating materials and of the intermediate products incl. transport to factory\nRecyclate re-granulation using ground material incl. transport to Viechtach\nEnergy supply for production\nProduction and packaging of the pipe system at the Viechtach factory\nInternal reprocessing of production waste and feedback into production\nRecycling of other waste incl. transport \nA4 – A5 Set-up phase\nTransport of product to construction site\nInstallation of pipe system\nRecycling of product packaging \nB use phase\nDeployment of pipe system (B1)\nMaintenance of pipe system (B2) \nC1 – C4 Disposal\nThree 100% disposal scenarios are assumed:\nEnd-of-Life (EoL) scenario 1: 100% dismantling of pipe system and thermal utilisation (module C3/1 and D/1).\nEoL scenario 2: 100% dismantling of pipe system and energetic utilisation (module C3/2 and D/2). \n\nEoL scenario 3: 100% dismantling of pipe system and energetic utilisation (module C4/3 and D/3) \n\nD Reuse, recovery and/or recycling potentials \nReuse, recovery and/or recycling potentials exist in the disposal scenarios because here, the pipe systems are put to energetic or material utilisation with recovery of energy or secondary materials which can then be used outside the system boundary.", "lang": "en"}], "other": {"anies": [{"name": "referenceToOriginalEPD", "value": {"shortDescription": {"value": "AWADUKT nevoPP SN10.pdf", "defaultValue": "AWADUKT nevoPP SN10.pdf", "lstrings": [{"lang": "de", "value": "AWADUKT nevoPP SN10.pdf"}]}, "type": "source data set", "uuid": {"uuid": "e9d4a492-ccc4-435b-9c3d-463f2240ce87"}, "refObjectId": "e9d4a492-ccc4-435b-9c3d-463f2240ce87", "resourceURLs": ["https://oekobaudat.de/OEKOBAU.DAT/resource/sources/e9d4a492-ccc4-435b-9c3d-463f2240ce87/AWADUKT_nevoPP_SN10_18929.pdf?version=00.01.000"]}}]}}, "validation": {"review": [{"referenceToNameOfReviewerAndInstitution": [{"shortDescription": [{"value": "Institut Bauen und Umwelt e. V.", "lang": "de"}], "type": "contact data set", "refObjectId": "d111dbec-b024-4be5-86c5-752d6eb2cf95", "uri": "../contacts/d111dbec-b024-4be5-86c5-752d6eb2cf95.xml"}], "type": "Accredited third party review"}]}, "complianceDeclarations": {"compliance": [{"referenceToComplianceSystem": {"shortDescription": [{"value": "DIN EN 15804+A2", "lang": "de"}], "type": "source data set", "refObjectId": "c0016b33-8cf7-415c-ac6e-deba0d21440d", "uri": "../sources/c0016b33-8cf7-415c-ac6e-deba0d21440d.xml"}}, {"referenceToComplianceSystem": {"shortDescription": [{"value": "ISO 14025", "lang": "de"}], "type": "source data set", "refObjectId": "4f2eb655-6e44-4874-a95a-e28f5442cd4d", "uri": "../sources/4f2eb655-6e44-4874-a95a-e28f5442cd4d.xml"}}]}}, "administrativeInformation": {"commissionerAndGoal": {"referenceToCommissioner": [{"shortDescription": [{"value": "REHAU Industries SE & Co. KG", "lang": "de"}], "type": "contact data set", "refObjectId": "b1b59d51-66a3-4983-acd8-86ad04e48050", "uri": "../contacts/b1b59d51-66a3-4983-acd8-86ad04e48050.xml"}]}, "dataGenerator": {"referenceToPersonOrEntityGeneratingTheDataSet": [{"shortDescription": [{"value": "SKZ - Das Kunststoff-Zentrum", "lang": "de"}], "type": "contact data set", "refObjectId": "2da43b2d-777d-45c6-ba4b-76c55a616a00", "uri": "../contacts/2da43b2d-777d-45c6-ba4b-76c55a616a00.xml"}]}, "dataEntryBy": {"timeStamp": 1720396800000, "referenceToDataSetFormat": [{"shortDescription": [{"value": "ILCD Format", "lang": "de"}], "type": "source data set", "refObjectId": "a97a0155-0234-4b87-b4ce-a45da52f2a40", "uri": "../sources/a97a0155-0234-4b87-b4ce-a45da52f2a40.xml"}, {"shortDescription": [{"value": "EPD-Datenformaterweiterungen v1.2", "lang": "de"}, {"value": "EPD Data Format Extensions v1.2", "lang": "en"}], "type": "source data set", "refObjectId": "a29449fd-aa2f-4de8-b5d7-4b06b43c6fde", "uri": "../sources/a29449fd-aa2f-4de8-b5d7-4b06b43c6fde.xml"}]}, "publicationAndOwnership": {"dataSetVersion": "00.01.000", "referenceToRegistrationAuthority": {"shortDescription": [{"value": "Institut Bauen und Umwelt e. V.", "lang": "de"}], "type": "contact data set", "refObjectId": "d111dbec-b024-4be5-86c5-752d6eb2cf95", "uri": "../contacts/d111dbec-b024-4be5-86c5-752d6eb2cf95.xml"}, "registrationNumber": "EPD-REH-20240086-ICC1-DE", "referenceToOwnershipOfDataSet": {"shortDescription": [{"value": "REHAU Industries SE & Co. KG", "lang": "de"}], "type": "contact data set", "refObjectId": "b1b59d51-66a3-4983-acd8-86ad04e48050", "uri": "../contacts/b1b59d51-66a3-4983-acd8-86ad04e48050.xml"}, "copyright": true, "licenseType": "Free of charge for all users and uses", "accessRestrictions": [{"value": "None", "lang": "en"}], "other": {"anies": [{"name": "referenceToPublisher", "value": {"shortDescription": [{"value": "Institut Bauen und Umwelt e. V.", "lang": "de"}], "type": "contact data set", "refObjectId": "d111dbec-b024-4be5-86c5-752d6eb2cf95", "uri": "../contacts/d111dbec-b024-4be5-86c5-752d6eb2cf95.xml"}}]}}}, "exchanges": {"exchange": [{"dataSetInternalID": 0, "referenceToFlowDataSet": {"shortDescription": [{"value": "Rohrsystem", "lang": "de"}], "type": "flow data set", "refObjectId": "8177c5c8-b8a6-ecec-b483-d4c5ee8e7914", "uri": "../flows/8177c5c8-b8a6-ecec-b483-d4c5ee8e7914.xml"}, "meanAmount": 1.0, "referencesToDataSource": {}, "referenceFlow": true, "resolvedFlowVersion": "00.01.000", "resultingflowAmount": 1.0, "flowProperties": [{"name": [{"lang": "en", "value": "Mass"}, {"lang": "de", "value": "Masse"}], "uuid": "93a60a56-a3c8-11da-a746-0800200b9a66", "referenceFlowProperty": true, "meanValue": 1.0, "referenceUnit": "kg", "unitGroupUUID": "ad38d542-3fe9-439d-9b95-2f5f7752acaf"}], "materialProperties": [{"name": "gross density", "value": "900.0", "unit": "kg/m^3", "unitDescription": "kilograms per cubic metre"}, {"name": "linear density", "value": "10.68", "unit": "kg/m"}], "typeOfFlow": "Product flow", "classification": {"classHierarchy": "Kunststoffe / Rohre / Abwasserrohre", "name": "OEKOBAU.DAT"}}, {"dataSetInternalID": 1, "referenceToFlowDataSet": {"shortDescription": [{"value": "Erneuerbare Primärenergie als Energieträger (PERE)", "lang": "de"}, {"value": "Renewable primary energy as energy carrier (PERE)", "lang": "en"}], "type": "flow data set", "refObjectId": "20f32be5-0398-4288-9b6d-accddd195317", "uri": "../flows/20f32be5-0398-4288-9b6d-accddd195317.xml"}, "exchange direction": "INPUT", "other": {"anies": [{"name": "referenceToUnitGroupDataSet", "value": {"shortDescription": [{"value": "MJ", "lang": "de"}], "type": "unit group data set", "refObjectId": "93a60a57-a3c8-11da-a746-0800200c9a66", "uri": "../unitgroups/93a60a57-a3c8-11da-a746-0800200c9a66.xml"}}, {"value": "7.81780082966874", "module": "A1-A3"}, {"value": "0.740414895497105", "module": "A4"}, {"value": "0.0109652362674899", "module": "A5"}, {"value": "0", "module": "B1"}, {"value": "0.134498209259462", "module": "B2"}, {"value": "0", "module": "B6"}, {"value": "0", "module": "B7"}, {"value": "0.00125670222326031", "module": "C1"}, {"value": "0.00425793355348848", "module": "C2"}, {"value": "0.0667915839880558", "module": "C3", "scenario": "S1"}, {"value": "0.0965417460634476", "module": "C3", "scenario": "S2"}, {"value": "0.0926143699254811", "module": "C4"}, {"value": "-0.60790432834486", "module": "D", "scenario": "S1"}, {"value": "-5.92562621210392", "module": "D", "scenario": "S2"}, {"value": "-0.0848750757727128", "module": "D", "scenario": "S3"}]}, "resolvedFlowVersion": "38.00.000", "flowProperties": [], "typeOfFlow": "Other flow", "classification": {"classHierarchy": "Quantities", "name": "GaBiCategories"}}, {"dataSetInternalID": 2, "referenceToFlowDataSet": {"shortDescription": [{"value": "Erneuerbare Primärenergie zur stofflichen Nutzung (PERM)", "lang": "de"}, {"value": "Renewable primary energy resources as material utilization (PERM)", "lang": "en"}], "type": "flow data set", "refObjectId": "fb3ec0de-548d-4508-aea5-00b73bf6f702", "uri": "../flows/fb3ec0de-548d-4508-aea5-00b73bf6f702.xml"}, "exchange direction": "INPUT", "other": {"anies": [{"name": "referenceToUnitGroupDataSet", "value": {"shortDescription": [{"value": "MJ", "lang": "de"}], "type": "unit group data set", "refObjectId": "93a60a57-a3c8-11da-a746-0800200c9a66", "uri": "../unitgroups/93a60a57-a3c8-11da-a746-0800200c9a66.xml"}}, {"value": "0.705110352852695", "module": "A1-A3"}, {"value": "0", "module": "A4"}, {"value": "-0.703392", "module": "A5"}, {"value": "0", "module": "B1"}, {"value": "0", "module": "B2"}, {"value": "0", "module": "B6"}, {"value": "0", "module": "B7"}, {"value": "0", "module": "C1"}, {"value": "0", "module": "C2"}, {"value": "-0.0017183528526947", "module": "C3", "scenario": "S1"}, {"value": "-0.0017183528526947", "module": "C3", "scenario": "S2"}, {"value": "0", "module": "C4"}, {"value": "0", "module": "D", "scenario": "S1"}, {"value": "0", "module": "D", "scenario": "S2"}, {"value": "0", "module": "D", "scenario": "S3"}]}, "resolvedFlowVersion": "38.00.000", "flowProperties": [], "typeOfFlow": "Other flow", "classification": {"classHierarchy": "Quantities", "name": "GaBiCategories"}}, {"dataSetInternalID": 3, "referenceToFlowDataSet": {"shortDescription": [{"value": "Total erneuerbare Primärenergie (PERT)", "lang": "de"}, {"value": "Total use of renewable primary energy resources (PERT)", "lang": "en"}], "type": "flow data set", "refObjectId": "53f97275-fa8a-4cdd-9024-65936002acd0", "uri": "../flows/53f97275-fa8a-4cdd-9024-65936002acd0.xml"}, "exchange direction": "INPUT", "other": {"anies": [{"name": "referenceToUnitGroupDataSet", "value": {"shortDescription": [{"value": "MJ", "lang": "de"}], "type": "unit group data set", "refObjectId": "93a60a57-a3c8-11da-a746-0800200c9a66", "uri": "../unitgroups/93a60a57-a3c8-11da-a746-0800200c9a66.xml"}}, {"value": "8.52291118252143", "module": "A1-A3"}, {"value": "0.740414895497105", "module": "A4"}, {"value": "-0.69242676373251", "module": "A5"}, {"value": "0", "module": "B1"}, {"value": "0.134498209259462", "module": "B2"}, {"value": "0", "module": "B6"}, {"value": "0", "module": "B7"}, {"value": "0.00125670222326031", "module": "C1"}, {"value": "0.00425793355348848", "module": "C2"}, {"value": "0.0650732311353611", "module": "C3", "scenario": "S1"}, {"value": "0.0948233932107529", "module": "C3", "scenario": "S2"}, {"value": "0.0926143699254811", "module": "C4"}, {"value": "-0.60790432834486", "module": "D", "scenario": "S1"}, {"value": "-0.00577010277191498", "module": "D", "scenario": "S2"}, {"value": "-2.64650057794538E-10", "module": "D", "scenario": "S3"}]}, "resolvedFlowVersion": "38.00.000", "flowProperties": [], "typeOfFlow": "Other flow", "classification": {"classHierarchy": "Quantities / Environmental quantities / EPD EN 15804 / LCI indicators", "name": "GaBiCategories"}}, {"dataSetInternalID": 4, "referenceToFlowDataSet": {"shortDescription": [{"value": "Nicht-erneuerbare Primärenergie als Energieträger (PENRE)", "lang": "de"}, {"value": "Non renewable primary energy as energy carrier (PENRE)", "lang": "en"}], "type": "flow data set", "refObjectId": "ac857178-2b45-46ec-892a-a9a4332f0372", "uri": "../flows/ac857178-2b45-46ec-892a-a9a4332f0372.xml"}, "exchange direction": "INPUT", "other": {"anies": [{"name": "referenceToUnitGroupDataSet", "value": {"shortDescription": [{"value": "MJ", "lang": "de"}], "type": "unit group data set", "refObjectId": "93a60a57-a3c8-11da-a746-0800200c9a66", "uri": "../unitgroups/93a60a57-a3c8-11da-a746-0800200c9a66.xml"}}, {"value": "18.0918974310019", "module": "A1-A3"}, {"value": "0.553247207624775", "module": "A4"}, {"value": "0.0811093066080413", "module": "A5"}, {"value": "0", "module": "B1"}, {"value": "2.30971472637842", "module": "B2"}, {"value": "0", "module": "B6"}, {"value": "0", "module": "B7"}, {"value": "0.0175805574679958", "module": "C1"}, {"value": "0.0587298978097998", "module": "C2"}, {"value": "1.72531199557712", "module": "C3", "scenario": "S1"}, {"value": "7.50766209038599", "module": "C3", "scenario": "S2"}, {"value": "1.02696003903421", "module": "C4"}, {"value": "-6.70450356726072", "module": "D", "scenario": "S1"}, {"value": "-26.5730488800371", "module": "D", "scenario": "S2"}, {"value": "-0.443043381951894", "module": "D", "scenario": "S3"}]}, "resolvedFlowVersion": "38.00.000", "flowProperties": [], "typeOfFlow": "Other flow", "classification": {"classHierarchy": "Quantities", "name": "GaBiCategories"}}, {"dataSetInternalID": 5, "referenceToFlowDataSet": {"shortDescription": [{"value": "Nicht-erneuerbare Primärenergie zur stofflichen Nutzung (PENRM)", "lang": "de"}, {"value": "Non renewable primary energy as material utilization (PENRM)", "lang": "en"}], "type": "flow data set", "refObjectId": "1421caa0-679d-4bf4-b282-0eb850ccae27", "uri": "../flows/1421caa0-679d-4bf4-b282-0eb850ccae27.xml"}, "exchange direction": "INPUT", "other": {"anies": [{"name": "referenceToUnitGroupDataSet", "value": {"shortDescription": [{"value": "MJ", "lang": "de"}], "type": "unit group data set", "refObjectId": "93a60a57-a3c8-11da-a746-0800200c9a66", "uri": "../unitgroups/93a60a57-a3c8-11da-a746-0800200c9a66.xml"}}, {"value": "7.13514914708902", "module": "A1-A3"}, {"value": "0", "module": "A4"}, {"value": "0.000187333824592709", "module": "A5"}, {"value": "0", "module": "B1"}, {"value": "0", "module": "B2"}, {"value": "0", "module": "B6"}, {"value": "0", "module": "B7"}, {"value": "0", "module": "C1"}, {"value": "0", "module": "C2"}, {"value": "-7.13533648091362", "module": "C3", "scenario": "S1"}, {"value": "-7.13533648091362", "module": "C3", "scenario": "S2"}, {"value": "0", "module": "C4"}, {"value": "0", "module": "D", "scenario": "S1"}, {"value": "0", "module": "D", "scenario": "S2"}, {"value": "0", "module": "D", "scenario": "S3"}]}, "resolvedFlowVersion": "38.00.000", "flowProperties": [], "typeOfFlow": "Other flow", "classification": {"classHierarchy": "Quantities", "name": "GaBiCategories"}}, {"dataSetInternalID": 6, "referenceToFlowDataSet": {"shortDescription": [{"value": "Total nicht erneuerbare Primärenergie (PENRT)", "lang": "de"}, {"value": "Total use of non renewable primary energy resources (PENRT)", "lang": "en"}], "type": "flow data set", "refObjectId": "06159210-646b-4c8d-8583-da9b3b95a6c1", "uri": "../flows/06159210-646b-4c8d-8583-da9b3b95a6c1.xml"}, "exchange direction": "INPUT", "other": {"anies": [{"name": "referenceToUnitGroupDataSet", "value": {"shortDescription": [{"value": "MJ", "lang": "de"}], "type": "unit group data set", "refObjectId": "93a60a57-a3c8-11da-a746-0800200c9a66", "uri": "../unitgroups/93a60a57-a3c8-11da-a746-0800200c9a66.xml"}}, {"value": "25.2270465780909", "module": "A1-A3"}, {"value": "0.553247207624775", "module": "A4"}, {"value": "0.081296640432634", "module": "A5"}, {"value": "0", "module": "B1"}, {"value": "2.30971472637842", "module": "B2"}, {"value": "0", "module": "B6"}, {"value": "0", "module": "B7"}, {"value": "0.0175805574679958", "module": "C1"}, {"value": "0.0587298978097998", "module": "C2"}, {"value": "-5.41002448533649", "module": "C3", "scenario": "S1"}, {"value": "0.372325609472378", "module": "C3", "scenario": "S2"}, {"value": "1.02696003903421", "module": "C4"}, {"value": "-6.70450356726072", "module": "D", "scenario": "S1"}, {"value": "-26.5730488800371", "module": "D", "scenario": "S2"}, {"value": "-0.443043381951894", "module": "D", "scenario": "S3"}]}, "resolvedFlowVersion": "38.00.000", "flowProperties": [], "typeOfFlow": "Other flow", "classification": {"classHierarchy": "Quantities / Environmental quantities / EPD EN 15804 / LCI indicators", "name": "GaBiCategories"}}, {"dataSetInternalID": 7, "referenceToFlowDataSet": {"shortDescription": [{"value": "Einsatz von Sekundärstoffen (SM)", "lang": "de"}, {"value": "Use of secondary material (SM)", "lang": "en"}], "type": "flow data set", "refObjectId": "c6a1f35f-2d09-4f54-8dfb-97e502e1ce92", "uri": "../flows/c6a1f35f-2d09-4f54-8dfb-97e502e1ce92.xml"}, "exchange direction": "INPUT", "other": {"anies": [{"name": "referenceToUnitGroupDataSet", "value": {"shortDescription": [{"value": "kg", "lang": "de"}], "type": "unit group data set", "refObjectId": "ad38d542-3fe9-439d-9b95-2f5f7752acaf", "uri": "../unitgroups/ad38d542-3fe9-439d-9b95-2f5f7752acaf.xml"}}, {"value": "0.8396129381228", "module": "A1-A3"}, {"value": "0", "module": "A4"}, {"value": "0", "module": "A5"}, {"value": "0", "module": "B1"}, {"value": "0", "module": "B2"}, {"value": "0", "module": "B6"}, {"value": "0", "module": "B7"}, {"value": "0", "module": "C1"}, {"value": "0", "module": "C2"}, {"value": "0", "module": "C3", "scenario": "S1"}, {"value": "0", "module": "C3", "scenario": "S2"}, {"value": "0", "module": "C4"}, {"value": "0.95", "module": "D", "scenario": "S1"}, {"value": "0", "module": "D", "scenario": "S2"}, {"value": "0", "module": "D", "scenario": "S3"}]}, "resolvedFlowVersion": "38.00.000", "flowProperties": [], "typeOfFlow": "Other flow", "classification": {"classHierarchy": "Quantities / Environmental quantities / EPD EN 15804 / LCI indicators", "name": "GaBiCategories"}}, {"dataSetInternalID": 8, "referenceToFlowDataSet": {"shortDescription": [{"value": "Erneuerbare Sekundärbrennstoffe (RSF)", "lang": "de"}, {"value": "Use of renewable secondary fuels (RSF)", "lang": "en"}], "type": "flow data set", "refObjectId": "64333088-a55f-4aa2-9a31-c10b07816787", "uri": "../flows/64333088-a55f-4aa2-9a31-c10b07816787.xml"}, "exchange direction": "INPUT", "other": {"anies": [{"name": "referenceToUnitGroupDataSet", "value": {"shortDescription": [{"value": "MJ", "lang": "de"}], "type": "unit group data set", "refObjectId": "93a60a57-a3c8-11da-a746-0800200c9a66", "uri": "../unitgroups/93a60a57-a3c8-11da-a746-0800200c9a66.xml"}}, {"value": "0", "module": "A1-A3"}, {"value": "0", "module": "A4"}, {"value": "0", "module": "A5"}, {"value": "0", "module": "B1"}, {"value": "0", "module": "B2"}, {"value": "0", "module": "B6"}, {"value": "0", "module": "B7"}, {"value": "0", "module": "C1"}, {"value": "0", "module": "C2"}, {"value": "0", "module": "C3", "scenario": "S1"}, {"value": "0", "module": "C3", "scenario": "S2"}, {"value": "0", "module": "C4"}, {"value": "0", "module": "D", "scenario": "S1"}, {"value": "0", "module": "D", "scenario": "S2"}, {"value": "0", "module": "D", "scenario": "S3"}]}, "resolvedFlowVersion": "38.00.000", "flowProperties": [], "typeOfFlow": "Other flow", "classification": {"classHierarchy": "Quantities / Environmental quantities / EPD EN 15804 / LCI indicators", "name": "GaBiCategories"}}, {"dataSetInternalID": 9, "referenceToFlowDataSet": {"shortDescription": [{"value": "Nicht erneuerbare Sekundärbrennstoffe (NRSF)", "lang": "de"}, {"value": "Use of non renewable secondary fuels (NRSF)", "lang": "en"}], "type": "flow data set", "refObjectId": "89def144-d39a-4287-b86f-efde453ddcb2", "uri": "../flows/89def144-d39a-4287-b86f-efde453ddcb2.xml"}, "exchange direction": "INPUT", "other": {"anies": [{"name": "referenceToUnitGroupDataSet", "value": {"shortDescription": [{"value": "MJ", "lang": "de"}], "type": "unit group data set", "refObjectId": "93a60a57-a3c8-11da-a746-0800200c9a66", "uri": "../unitgroups/93a60a57-a3c8-11da-a746-0800200c9a66.xml"}}, {"value": "0", "module": "A1-A3"}, {"value": "0", "module": "A4"}, {"value": "0", "module": "A5"}, {"value": "0", "module": "B1"}, {"value": "0", "module": "B2"}, {"value": "0", "module": "B6"}, {"value": "0", "module": "B7"}, {"value": "0", "module": "C1"}, {"value": "0", "module": "C2"}, {"value": "0", "module": "C3", "scenario": "S1"}, {"value": "0", "module": "C3", "scenario": "S2"}, {"value": "0", "module": "C4"}, {"value": "0", "module": "D", "scenario": "S1"}, {"value": "0", "module": "D", "scenario": "S2"}, {"value": "0", "module": "D", "scenario": "S3"}]}, "resolvedFlowVersion": "38.00.000", "flowProperties": [], "typeOfFlow": "Other flow", "classification": {"classHierarchy": "Quantities / Environmental quantities / EPD EN 15804 / LCI indicators", "name": "GaBiCategories"}}, {"dataSetInternalID": 10, "referenceToFlowDataSet": {"shortDescription": [{"value": "Einsatz von Süßwasserressourcen (FW)", "lang": "de"}, {"value": "Use of net fresh water (FW)", "lang": "en"}], "type": "flow data set", "refObjectId": "3cf952c8-f3a4-461d-8c96-96456ca62246", "uri": "../flows/3cf952c8-f3a4-461d-8c96-96456ca62246.xml"}, "exchange direction": "INPUT", "other": {"anies": [{"name": "referenceToUnitGroupDataSet", "value": {"shortDescription": [{"value": "m^3", "lang": "de"}], "type": "unit group data set", "refObjectId": "cd950537-0a98-4044-9ba7-9f9a68d0a504", "uri": "../unitgroups/cd950537-0a98-4044-9ba7-9f9a68d0a504.xml"}}, {"value": "0.00319475273265901", "module": "A1-A3"}, {"value": "3.29422607867793E-05", "module": "A4"}, {"value": "0.000210918358545274", "module": "A5"}, {"value": "0", "module": "B1"}, {"value": "0.000177997658773119", "module": "B2"}, {"value": "0", "module": "B6"}, {"value": "0", "module": "B7"}, {"value": "1.38086028208613E-06", "module": "C1"}, {"value": "4.66358482723763E-06", "module": "C2"}, {"value": "0.0020257358362329", "module": "C3", "scenario": "S1"}, {"value": "0.00676083556493426", "module": "C3", "scenario": "S2"}, {"value": "1.01259919015328E-05", "module": "C4"}, {"value": "-0.000902555930012428", "module": "D", "scenario": "S1"}, {"value": "-0.00577009680221829", "module": "D", "scenario": "S2"}, {"value": "-8.27311343161788E-05", "module": "D", "scenario": "S3"}]}, "resolvedFlowVersion": "38.00.000", "flowProperties": [], "typeOfFlow": "Other flow", "classification": {"classHierarchy": "Quantities / Environmental quantities / EPD EN 15804 / LCI indicators", "name": "GaBiCategories"}}, {"dataSetInternalID": 11, "referenceToFlowDataSet": {"shortDescription": [{"value": "Gefährlicher Abfall zur Deponie (HWD)", "lang": "de"}, {"value": "Hazardous waste disposed (HWD)", "lang": "en"}], "type": "flow data set", "refObjectId": "430f9e0f-59b2-46a0-8e0d-55e0e84948fc", "uri": "../flows/430f9e0f-59b2-46a0-8e0d-55e0e84948fc.xml"}, "exchange direction": "OUTPUT", "other": {"anies": [{"name": "referenceToUnitGroupDataSet", "value": {"shortDescription": [{"value": "kg", "lang": "de"}], "type": "unit group data set", "refObjectId": "ad38d542-3fe9-439d-9b95-2f5f7752acaf", "uri": "../unitgroups/ad38d542-3fe9-439d-9b95-2f5f7752acaf.xml"}}, {"value": "-6.40952687478573E-10", "module": "A1-A3"}, {"value": "9.32426268299211E-13", "module": "A4"}, {"value": "2.28732658161083E-13", "module": "A5"}, {"value": "0", "module": "B1"}, {"value": "-1.17158478041068E-11", "module": "B2"}, {"value": "0", "module": "B6"}, {"value": "0", "module": "B7"}, {"value": "6.00954926507276E-14", "module": "C1"}, {"value": "1.81846401594478E-13", "module": "C2"}, {"value": "4.45018378068291E-11", "module": "C3", "scenario": "S1"}, {"value": "8.37325424290522E-12", "module": "C3", "scenario": "S2"}, {"value": "8.64722300453677E-11", "module": "C4"}, {"value": "-7.7104601009773E-10", "module": "D", "scenario": "S1"}, {"value": "-5.96969668551806E-09", "module": "D", "scenario": "S2"}, {"value": "-9.71519544872693E-11", "module": "D", "scenario": "S3"}]}, "resolvedFlowVersion": "38.00.000", "flowProperties": [], "typeOfFlow": "Other flow", "classification": {"classHierarchy": "Quantities / Environmental quantities / EPD EN 15804 / LCI indicators", "name": "GaBiCategories"}}, {"dataSetInternalID": 12, "referenceToFlowDataSet": {"shortDescription": [{"value": "Entsorgter nicht gefährlicher Abfall (NHWD)", "lang": "de"}, {"value": "Non hazardous waste disposed (NHWD)", "lang": "en"}], "type": "flow data set", "refObjectId": "b29ef66b-e286-4afa-949f-62f1a7b4d7fa", "uri": "../flows/b29ef66b-e286-4afa-949f-62f1a7b4d7fa.xml"}, "exchange direction": "OUTPUT", "other": {"anies": [{"name": "referenceToUnitGroupDataSet", "value": {"shortDescription": [{"value": "kg", "lang": "de"}], "type": "unit group data set", "refObjectId": "ad38d542-3fe9-439d-9b95-2f5f7752acaf", "uri": "../unitgroups/ad38d542-3fe9-439d-9b95-2f5f7752acaf.xml"}}, {"value": "0.00814260243764259", "module": "A1-A3"}, {"value": "8.27885021088914E-05", "module": "A4"}, {"value": "0.00115710346345312", "module": "A5"}, {"value": "0", "module": "B1"}, {"value": "0.037183915098208", "module": "B2"}, {"value": "0", "module": "B6"}, {"value": "0", "module": "B7"}, {"value": "2.60202376521315E-06", "module": "C1"}, {"value": "8.9527355979454E-06", "module": "C2"}, {"value": "0.00142018944900822", "module": "C3", "scenario": "S1"}, {"value": "0.0124104149546883", "module": "C3", "scenario": "S2"}, {"value": "0.995825225188029", "module": "C4"}, {"value": "-0.00192729550521014", "module": "D", "scenario": "S1"}, {"value": "-0.0124033095334722", "module": "D", "scenario": "S2"}, {"value": "-0.000192536703154096", "module": "D", "scenario": "S3"}]}, "resolvedFlowVersion": "38.00.000", "flowProperties": [], "typeOfFlow": "Other flow", "classification": {"classHierarchy": "Quantities / Environmental quantities / EPD EN 15804 / LCI indicators", "name": "GaBiCategories"}}, {"dataSetInternalID": 13, "referenceToFlowDataSet": {"shortDescription": [{"value": "Entsorgter radioaktiver Abfall (RWD)", "lang": "de"}, {"value": "Radioactive waste disposed (RWD)", "lang": "en"}], "type": "flow data set", "refObjectId": "3449546e-52ad-4b39-b809-9fb77cea8ff6", "uri": "../flows/3449546e-52ad-4b39-b809-9fb77cea8ff6.xml"}, "exchange direction": "OUTPUT", "other": {"anies": [{"name": "referenceToUnitGroupDataSet", "value": {"shortDescription": [{"value": "kg", "lang": "de"}], "type": "unit group data set", "refObjectId": "ad38d542-3fe9-439d-9b95-2f5f7752acaf", "uri": "../unitgroups/ad38d542-3fe9-439d-9b95-2f5f7752acaf.xml"}}, {"value": "0.000258342134422482", "module": "A1-A3"}, {"value": "7.28123266935418E-07", "module": "A4"}, {"value": "8.23521432220183E-07", "module": "A5"}, {"value": "0", "module": "B1"}, {"value": "1.43154887140277E-05", "module": "B2"}, {"value": "0", "module": "B6"}, {"value": "0", "module": "B7"}, {"value": "2.74777027547017E-08", "module": "C1"}, {"value": "1.09909510597166E-07", "module": "C2"}, {"value": "0.000110431882296108", "module": "C3", "scenario": "S1"}, {"value": "2.24043562345365E-05", "module": "C3", "scenario": "S2"}, {"value": "1.21576770627837E-05", "module": "C4"}, {"value": "-0.000150180573639858", "module": "D", "scenario": "S1"}, {"value": "-0.00189811949815052", "module": "D", "scenario": "S2"}, {"value": "-2.71478210587265E-05", "module": "D", "scenario": "S3"}]}, "resolvedFlowVersion": "38.00.000", "flowProperties": [], "typeOfFlow": "Other flow", "classification": {"classHierarchy": "Quantities / Environmental quantities / EPD EN 15804 / LCI indicators", "name": "GaBiCategories"}}, {"dataSetInternalID": 14, "referenceToFlowDataSet": {"shortDescription": [{"value": "Komponenten für die Wiederverwendung (CRU)", "lang": "de"}, {"value": "Components for re-use (CRU)", "lang": "en"}], "type": "flow data set", "refObjectId": "a2b32f97-3fc7-4af2-b209-525bc6426f33", "uri": "../flows/a2b32f97-3fc7-4af2-b209-525bc6426f33.xml"}, "exchange direction": "OUTPUT", "other": {"anies": [{"name": "referenceToUnitGroupDataSet", "value": {"shortDescription": [{"value": "kg", "lang": "de"}], "type": "unit group data set", "refObjectId": "ad38d542-3fe9-439d-9b95-2f5f7752acaf", "uri": "../unitgroups/ad38d542-3fe9-439d-9b95-2f5f7752acaf.xml"}}, {"value": "0", "module": "A1-A3"}, {"value": "0", "module": "A4"}, {"value": "0", "module": "A5"}, {"value": "0", "module": "B1"}, {"value": "0", "module": "B2"}, {"value": "0", "module": "B6"}, {"value": "0", "module": "B7"}, {"value": "0", "module": "C1"}, {"value": "0", "module": "C2"}, {"value": "0", "module": "C3", "scenario": "S1"}, {"value": "0", "module": "C3", "scenario": "S2"}, {"value": "0", "module": "C4"}, {"value": "0", "module": "D", "scenario": "S1"}, {"value": "0", "module": "D", "scenario": "S2"}, {"value": "0", "module": "D", "scenario": "S3"}]}, "resolvedFlowVersion": "38.00.000", "flowProperties": [], "typeOfFlow": "Other flow", "classification": {"classHierarchy": "Quantities / Environmental quantities / EPD EN 15804 / LCI indicators", "name": "GaBiCategories"}}, {"dataSetInternalID": 15, "referenceToFlowDataSet": {"shortDescription": [{"value": "Stoffe zum Recycling (MFR)", "lang": "de"}, {"value": "Materials for recycling (MFR)", "lang": "en"}], "type": "flow data set", "refObjectId": "d7fe48a5-4103-49c8-9aae-b0b5dfdbd6ae", "uri": "../flows/d7fe48a5-4103-49c8-9aae-b0b5dfdbd6ae.xml"}, "exchange direction": "OUTPUT", "other": {"anies": [{"name": "referenceToUnitGroupDataSet", "value": {"shortDescription": [{"value": "kg", "lang": "de"}], "type": "unit group data set", "refObjectId": "ad38d542-3fe9-439d-9b95-2f5f7752acaf", "uri": "../unitgroups/ad38d542-3fe9-439d-9b95-2f5f7752acaf.xml"}}, {"value": "0.0354129381227999", "module": "A1-A3"}, {"value": "0", "module": "A4"}, {"value": "0.000216959921135779", "module": "A5"}, {"value": "0", "module": "B1"}, {"value": "0", "module": "B2"}, {"value": "0", "module": "B6"}, {"value": "0", "module": "B7"}, {"value": "0", "module": "C1"}, {"value": "0", "module": "C2"}, {"value": "0.949783040078864", "module": "C3", "scenario": "S1"}, {"value": "0", "module": "C3", "scenario": "S2"}, {"value": "0", "module": "C4"}, {"value": "0", "module": "D", "scenario": "S1"}, {"value": "0", "module": "D", "scenario": "S2"}, {"value": "0", "module": "D", "scenario": "S3"}]}, "resolvedFlowVersion": "38.00.000", "flowProperties": [], "typeOfFlow": "Other flow", "classification": {"classHierarchy": "Quantities / Environmental quantities / EPD EN 15804 / LCI indicators", "name": "GaBiCategories"}}, {"dataSetInternalID": 16, "referenceToFlowDataSet": {"shortDescription": [{"value": "Stoffe für die Energierückgewinnung (MER)", "lang": "de"}, {"value": "Materials for energy recovery (MER)", "lang": "en"}], "type": "flow data set", "refObjectId": "59a9181c-3aaf-46ee-8b13-2b3723b6e447", "uri": "../flows/59a9181c-3aaf-46ee-8b13-2b3723b6e447.xml"}, "exchange direction": "OUTPUT", "other": {"anies": [{"name": "referenceToUnitGroupDataSet", "value": {"shortDescription": [{"value": "kg", "lang": "de"}], "type": "unit group data set", "refObjectId": "ad38d542-3fe9-439d-9b95-2f5f7752acaf", "uri": "../unitgroups/ad38d542-3fe9-439d-9b95-2f5f7752acaf.xml"}}, {"value": "0", "module": "A1-A3"}, {"value": "0", "module": "A4"}, {"value": "0", "module": "A5"}, {"value": "0", "module": "B1"}, {"value": "0", "module": "B2"}, {"value": "0", "module": "B6"}, {"value": "0", "module": "B7"}, {"value": "0", "module": "C1"}, {"value": "0", "module": "C2"}, {"value": "0", "module": "C3", "scenario": "S1"}, {"value": "0", "module": "C3", "scenario": "S2"}, {"value": "0", "module": "C4"}, {"value": "0", "module": "D", "scenario": "S1"}, {"value": "0", "module": "D", "scenario": "S2"}, {"value": "0", "module": "D", "scenario": "S3"}]}, "resolvedFlowVersion": "38.00.000", "flowProperties": [], "typeOfFlow": "Other flow", "classification": {"classHierarchy": "Quantities / Environmental quantities / EPD EN 15804 / LCI indicators", "name": "GaBiCategories"}}, {"dataSetInternalID": 17, "referenceToFlowDataSet": {"shortDescription": [{"value": "Exportierte elektrische Energie (EEE)", "lang": "de"}, {"value": "Exported electrical energy (EEE)", "lang": "en"}], "type": "flow data set", "refObjectId": "4da0c987-2b76-40d6-9e9e-82a017aaaf29", "uri": "../flows/4da0c987-2b76-40d6-9e9e-82a017aaaf29.xml"}, "exchange direction": "OUTPUT", "other": {"anies": [{"name": "referenceToUnitGroupDataSet", "value": {"shortDescription": [{"value": "MJ", "lang": "de"}], "type": "unit group data set", "refObjectId": "93a60a57-a3c8-11da-a746-0800200c9a66", "uri": "../unitgroups/93a60a57-a3c8-11da-a746-0800200c9a66.xml"}}, {"value": "0.0486", "module": "A1-A3"}, {"value": "0", "module": "A4"}, {"value": "0.0968", "module": "A5"}, {"value": "0", "module": "B1"}, {"value": "0", "module": "B2"}, {"value": "0", "module": "B6"}, {"value": "0", "module": "B7"}, {"value": "0", "module": "C1"}, {"value": "0", "module": "C2"}, {"value": "0.334", "module": "C3", "scenario": "S1"}, {"value": "6.68113999843291", "module": "C3", "scenario": "S2"}, {"value": "0", "module": "C4"}, {"value": "0", "module": "D", "scenario": "S1"}, {"value": "0", "module": "D", "scenario": "S2"}, {"value": "0", "module": "D", "scenario": "S3"}]}, "resolvedFlowVersion": "38.00.000", "flowProperties": [], "typeOfFlow": "Other flow", "classification": {"classHierarchy": "Quantities / Environmental quantities / EPD EN 15804 / LCI indicators", "name": "GaBiCategories"}}, {"dataSetInternalID": 18, "referenceToFlowDataSet": {"shortDescription": [{"value": "Exportierte thermische Energie (EET)", "lang": "de"}, {"value": "Exported thermal energy (EET)", "lang": "en"}], "type": "flow data set", "refObjectId": "98daf38a-7a79-46d3-9a37-2b7bd0955810", "uri": "../flows/98daf38a-7a79-46d3-9a37-2b7bd0955810.xml"}, "exchange direction": "OUTPUT", "other": {"anies": [{"name": "referenceToUnitGroupDataSet", "value": {"shortDescription": [{"value": "MJ", "lang": "de"}], "type": "unit group data set", "refObjectId": "93a60a57-a3c8-11da-a746-0800200c9a66", "uri": "../unitgroups/93a60a57-a3c8-11da-a746-0800200c9a66.xml"}}, {"value": "0.0112", "module": "A1-A3"}, {"value": "0", "module": "A4"}, {"value": "0.228", "module": "A5"}, {"value": "0", "module": "B1"}, {"value": "0", "module": "B2"}, {"value": "0", "module": "B6"}, {"value": "0", "module": "B7"}, {"value": "0", "module": "C1"}, {"value": "0", "module": "C2"}, {"value": "0.594", "module": "C3", "scenario": "S1"}, {"value": "11.8799848225502", "module": "C3", "scenario": "S2"}, {"value": "0", "module": "C4"}, {"value": "0", "module": "D", "scenario": "S1"}, {"value": "0", "module": "D", "scenario": "S2"}, {"value": "0", "module": "D", "scenario": "S3"}]}, "resolvedFlowVersion": "38.00.000", "flowProperties": [], "typeOfFlow": "Other flow", "classification": {"classHierarchy": "Quantities / Environmental quantities / EPD EN 15804 / LCI indicators", "name": "GaBiCategories"}}]}, "LCIAResults": {"LCIAResult": [{"referenceToLCIAMethodDataSet": {"shortDescription": [{"value": "Globales Erwärmungspotenzial total (GWP-total)", "lang": "de"}, {"value": "Global Warming Potential total (GWP-total)", "lang": "en"}], "type": "LCIA method data set", "refObjectId": "6a37f984-a4b3-458a-a20a-64418c145fa2", "uri": "../lciamethods/6a37f984-a4b3-458a-a20a-64418c145fa2.xml"}, "other": {"anies": [{"name": "referenceToUnitGroupDataSet", "value": {"shortDescription": [{"value": "kg CO_(2)-Äq.", "lang": "de"}], "type": "unit group data set", "refObjectId": "1ebf3012-d0db-4de2-aefd-ef30cedb0be1", "uri": "../unitgroups/1ebf3012-d0db-4de2-aefd-ef30cedb0be1.xml"}}, {"value": "0.742366855441622", "module": "A1-A3"}, {"value": "0.040493315647015", "module": "A4"}, {"value": "0.0822560461463946", "module": "A5"}, {"value": "0", "module": "B1"}, {"value": "0.199228514195419", "module": "B2"}, {"value": "0", "module": "B6"}, {"value": "0", "module": "B7"}, {"value": "0.00130422959038152", "module": "C1"}, {"value": "0.0042930345073031", "module": "C2"}, {"value": "0.246285767093526", "module": "C3", "scenario": "S1"}, {"value": "3.12937036354547", "module": "C3", "scenario": "S2"}, {"value": "0.0677379410827289", "module": "C4"}, {"value": "-0.222779552309522", "module": "D", "scenario": "S1"}, {"value": "-1.52132309116838", "module": "D", "scenario": "S2"}, {"value": "-0.0254313885633405", "module": "D", "scenario": "S3"}]}}, {"referenceToLCIAMethodDataSet": {"shortDescription": [{"value": "Globales Erwärmungspotenzial fossil (GWP-fossil)", "lang": "de"}, {"value": "Global Warming Potential fossil fuels (GWP-fossil)", "lang": "en"}], "type": "LCIA method data set", "refObjectId": "5f635281-343e-44fb-83df-1971b155e6b6", "uri": "../lciamethods/5f635281-343e-44fb-83df-1971b155e6b6.xml"}, "other": {"anies": [{"name": "referenceToUnitGroupDataSet", "value": {"shortDescription": [{"value": "kg CO_(2)-Äq.", "lang": "de"}], "type": "unit group data set", "refObjectId": "1ebf3012-d0db-4de2-aefd-ef30cedb0be1", "uri": "../unitgroups/1ebf3012-d0db-4de2-aefd-ef30cedb0be1.xml"}}, {"value": "0.809406356096005", "module": "A1-A3"}, {"value": "0.0401362970736785", "module": "A4"}, {"value": "0.00575318778495028", "module": "A5"}, {"value": "0", "module": "B1"}, {"value": "0.179178740344873", "module": "B2"}, {"value": "0", "module": "B6"}, {"value": "0", "module": "B7"}, {"value": "0.00129974612141028", "module": "C1"}, {"value": "0.00424354280334609", "module": "C2"}, {"value": "0.246232161598498", "module": "C3", "scenario": "S1"}, {"value": "3.12928361331611", "module": "C3", "scenario": "S2"}, {"value": "0.0685267076788917", "module": "C4"}, {"value": "-0.221599384494232", "module": "D", "scenario": "S1"}, {"value": "-1.51416573052276", "module": "D", "scenario": "S2"}, {"value": "-0.0253233611950389", "module": "D", "scenario": "S3"}]}}, {"referenceToLCIAMethodDataSet": {"shortDescription": [{"value": "Globales Erwärmungspotenzial biogen (GWP-biogenic)", "lang": "de"}, {"value": "Global Warming Potential biogenic (GWP-biogenic)", "lang": "en"}], "type": "LCIA method data set", "refObjectId": "2356e1ab-0185-4db5-86e5-16de51c7485c", "uri": "../lciamethods/2356e1ab-0185-4db5-86e5-16de51c7485c.xml"}, "other": {"anies": [{"name": "referenceToUnitGroupDataSet", "value": {"shortDescription": [{"value": "kg CO_(2)-Äq.", "lang": "de"}], "type": "unit group data set", "refObjectId": "1ebf3012-d0db-4de2-aefd-ef30cedb0be1", "uri": "../unitgroups/1ebf3012-d0db-4de2-aefd-ef30cedb0be1.xml"}}, {"value": "-0.0676732089014763", "module": "A1-A3"}, {"value": "0.00011408487203579", "module": "A4"}, {"value": "0.0764764160990038", "module": "A5"}, {"value": "0", "module": "B1"}, {"value": "0.0200394132965335", "module": "B2"}, {"value": "0", "module": "B6"}, {"value": "0", "module": "B7"}, {"value": "0", "module": "C1"}, {"value": "9.71386801035436E-06", "module": "C2"}, {"value": "4.52870795101933E-05", "module": "C3", "scenario": "S1"}, {"value": "8.36597871207117E-05", "module": "C3", "scenario": "S2"}, {"value": "0", "module": "C4"}, {"value": "-0.0010951005403859", "module": "D", "scenario": "S1"}, {"value": "-0.00610687196628068", "module": "D", "scenario": "S2"}, {"value": "-9.28866341021704E-05", "module": "D", "scenario": "S3"}]}}, {"referenceToLCIAMethodDataSet": {"shortDescription": [{"value": "Globales Erwärmungspotenzial luluc (GWP-luluc)", "lang": "de"}, {"value": "Global Warming Potential luluc (GWP-luluc)", "lang": "en"}], "type": "LCIA method data set", "refObjectId": "4331bbdb-978a-490d-8707-eeb047f01a55", "uri": "../lciamethods/4331bbdb-978a-490d-8707-eeb047f01a55.xml"}, "other": {"anies": [{"name": "referenceToUnitGroupDataSet", "value": {"shortDescription": [{"value": "kg CO_(2)-Äq.", "lang": "de"}], "type": "unit group data set", "refObjectId": "1ebf3012-d0db-4de2-aefd-ef30cedb0be1", "uri": "../unitgroups/1ebf3012-d0db-4de2-aefd-ef30cedb0be1.xml"}}, {"value": "0.000633708247092857", "module": "A1-A3"}, {"value": "0.000242933701300684", "module": "A4"}, {"value": "2.64422624405719E-05", "module": "A5"}, {"value": "0", "module": "B1"}, {"value": "1.03605540127485E-05", "module": "B2"}, {"value": "0", "module": "B6"}, {"value": "0", "module": "B7"}, {"value": "1.1926640617035E-05", "module": "C1"}, {"value": "3.97778359466603E-05", "module": "C2"}, {"value": "8.31841551766863E-06", "module": "C3", "scenario": "S1"}, {"value": "3.09044223481775E-06", "module": "C3", "scenario": "S2"}, {"value": "5.65939994740502E-05", "module": "C4"}, {"value": "-8.50672749040527E-05", "module": "D", "scenario": "S1"}, {"value": "-0.00105048867934252", "module": "D", "scenario": "S2"}, {"value": "-1.51407341994144E-05", "module": "D", "scenario": "S3"}]}}, {"referenceToLCIAMethodDataSet": {"shortDescription": [{"value": "Abbau Potential der stratosphärischen Ozonschicht (ODP)", "lang": "de"}, {"value": "Depletion potential of the stratospheric ozone layer (ODP)", "lang": "en"}], "type": "LCIA method data set", "refObjectId": "b5c629d6-def3-11e6-bf01-fe55135034f3", "uri": "../lciamethods/b5c629d6-def3-11e6-bf01-fe55135034f3.xml"}, "other": {"anies": [{"name": "referenceToUnitGroupDataSet", "value": {"shortDescription": [{"value": "kg CFC11-Äq.", "lang": "de"}], "type": "unit group data set", "refObjectId": "d9e957c9-7309-4474-bf3a-7777df6c4e5b", "uri": "../unitgroups/d9e957c9-7309-4474-bf3a-7777df6c4e5b.xml"}}, {"value": "1.55692110738799E-11", "module": "A1-A3"}, {"value": "1.00198407929494E-14", "module": "A4"}, {"value": "1.53460388285289E-14", "module": "A5"}, {"value": "0", "module": "B1"}, {"value": "2.72271637705519E-13", "module": "B2"}, {"value": "0", "module": "B6"}, {"value": "0", "module": "B7"}, {"value": "1.382888393025E-16", "module": "C1"}, {"value": "5.58851970874669E-16", "module": "C2"}, {"value": "1.23877843718712E-14", "module": "C3", "scenario": "S1"}, {"value": "1.4813560132544E-13", "module": "C3", "scenario": "S2"}, {"value": "1.15543667059256E-13", "module": "C4"}, {"value": "-4.36413221145274E-13", "module": "D", "scenario": "S1"}, {"value": "-1.7284848316353E-14", "module": "D", "scenario": "S2"}, {"value": "-2.47308076605434E-16", "module": "D", "scenario": "S3"}]}}, {"referenceToLCIAMethodDataSet": {"shortDescription": [{"value": "Versauerungspotenzial von Boden und Wasser (AP)", "lang": "de"}, {"value": "Acidification potential of land and water (AP)", "lang": "en"}], "type": "LCIA method data set", "refObjectId": "b5c611c6-def3-11e6-bf01-fe55135034f3", "uri": "../lciamethods/b5c611c6-def3-11e6-bf01-fe55135034f3.xml"}, "other": {"anies": [{"name": "referenceToUnitGroupDataSet", "value": {"shortDescription": [{"value": "mol H^(+)-Äq.", "lang": "de"}], "type": "unit group data set", "refObjectId": "42e089ac-92bf-4bf2-8ca1-5fc40d18f2ed", "uri": "../unitgroups/42e089ac-92bf-4bf2-8ca1-5fc40d18f2ed.xml"}}, {"value": "0.00137132725323188", "module": "A1-A3"}, {"value": "5.45544979657274E-05", "module": "A4"}, {"value": "2.03016778137608E-05", "module": "A5"}, {"value": "0", "module": "B1"}, {"value": "0.000215514620248796", "module": "B2"}, {"value": "0", "module": "B6"}, {"value": "0", "module": "B7"}, {"value": "6.65824920855279E-06", "module": "C1"}, {"value": "6.40262721370512E-06", "module": "C2"}, {"value": "0.000168208360853876", "module": "C3", "scenario": "S1"}, {"value": "0.000308679580636112", "module": "C3", "scenario": "S2"}, {"value": "0.000206253740908258", "module": "C4"}, {"value": "-0.000309857380440897", "module": "D", "scenario": "S1"}, {"value": "-0.00198418566678015", "module": "D", "scenario": "S2"}, {"value": "-3.06131915420542E-05", "module": "D", "scenario": "S3"}]}}, {"referenceToLCIAMethodDataSet": {"shortDescription": [{"value": "Eutrophierungspotenzial Süßwasser (EP-freshwater)", "lang": "de"}, {"value": "Eutrophication potential aquatic freshwater (EP-freshwater)", "lang": "en"}], "type": "LCIA method data set", "refObjectId": "b53ec18f-7377-4ad3-86eb-cc3f4f276b2b", "uri": "../lciamethods/b53ec18f-7377-4ad3-86eb-cc3f4f276b2b.xml"}, "other": {"anies": [{"name": "referenceToUnitGroupDataSet", "value": {"shortDescription": [{"value": "kg P-Äq.", "lang": "de"}], "type": "unit group data set", "refObjectId": "0429039d-a61d-4590-ba67-aa4a20a810a1", "uri": "../unitgroups/0429039d-a61d-4590-ba67-aa4a20a810a1.xml"}}, {"value": "3.78932155912021E-06", "module": "A1-A3"}, {"value": "9.57279266138524E-08", "module": "A4"}, {"value": "1.40276006895242E-08", "module": "A5"}, {"value": "0", "module": "B1"}, {"value": "2.3365315783951E-05", "module": "B2"}, {"value": "0", "module": "B6"}, {"value": "0", "module": "B7"}, {"value": "4.70143470297397E-09", "module": "C1"}, {"value": "1.57029690637775E-08", "module": "C2"}, {"value": "4.41935149559539E-08", "module": "C3", "scenario": "S1"}, {"value": "3.51340777942033E-08", "module": "C3", "scenario": "S2"}, {"value": "1.32342529672598E-05", "module": "C4"}, {"value": "-3.08999962325862E-07", "module": "D", "scenario": "S1"}, {"value": "-1.98533298832406E-06", "module": "D", "scenario": "S2"}, {"value": "-2.859800768507E-08", "module": "D", "scenario": "S3"}]}}, {"referenceToLCIAMethodDataSet": {"shortDescription": [{"value": "Eutrophierungspotenzial Salzwasser (EP-marine)", "lang": "de"}, {"value": "Eutrophication potential aquatic marine (EP-marine)", "lang": "en"}], "type": "LCIA method data set", "refObjectId": "b5c619fa-def3-11e6-bf01-fe55135034f3", "uri": "../lciamethods/b5c619fa-def3-11e6-bf01-fe55135034f3.xml"}, "other": {"anies": [{"name": "referenceToUnitGroupDataSet", "value": {"shortDescription": [{"value": "kg N-Äq.", "lang": "de"}], "type": "unit group data set", "refObjectId": "d05bb823-ecdf-4686-8c40-bf1d9257859f", "uri": "../unitgroups/d05bb823-ecdf-4686-8c40-bf1d9257859f.xml"}}, {"value": "0.000386854221673694", "module": "A1-A3"}, {"value": "2.04545808206394E-05", "module": "A4"}, {"value": "5.38786563280027E-06", "module": "A5"}, {"value": "0", "module": "B1"}, {"value": "0.000166836566492712", "module": "B2"}, {"value": "0", "module": "B6"}, {"value": "0", "module": "B7"}, {"value": "3.12862852610377E-06", "module": "C1"}, {"value": "2.33505159026185E-06", "module": "C2"}, {"value": "4.3476426889453E-05", "module": "C3", "scenario": "S1"}, {"value": "6.46694061471306E-05", "module": "C3", "scenario": "S2"}, {"value": "4.72497806533435E-05", "module": "C4"}, {"value": "-8.90498532233837E-05", "module": "D", "scenario": "S1"}, {"value": "-0.00056668671898092", "module": "D", "scenario": "S2"}, {"value": "-9.0692265811587E-06", "module": "D", "scenario": "S3"}]}}, {"referenceToLCIAMethodDataSet": {"shortDescription": [{"value": "Eutrophierungspotenzial Land (EP-terrestrial)", "lang": "de"}, {"value": "Eutrophication potential terrestrial (EP-terrestrial)", "lang": "en"}], "type": "LCIA method data set", "refObjectId": "b5c614d2-def3-11e6-bf01-fe55135034f3", "uri": "../lciamethods/b5c614d2-def3-11e6-bf01-fe55135034f3.xml"}, "other": {"anies": [{"name": "referenceToUnitGroupDataSet", "value": {"shortDescription": [{"value": "mol N-Äq.", "lang": "de"}], "type": "unit group data set", "refObjectId": "71b4d617-0ec9-4d3f-b65e-e438940c2401", "uri": "../unitgroups/71b4d617-0ec9-4d3f-b65e-e438940c2401.xml"}}, {"value": "0.00410758254462715", "module": "A1-A3"}, {"value": "0.000241889613104815", "module": "A4"}, {"value": "8.57932136532527E-05", "module": "A5"}, {"value": "0", "module": "B1"}, {"value": "0.000826393663451446", "module": "B2"}, {"value": "0", "module": "B6"}, {"value": "0", "module": "B7"}, {"value": "3.46703883129639E-05", "module": "C1"}, {"value": "2.7602604301917E-05", "module": "C2"}, {"value": "0.000508783904402987", "module": "C3", "scenario": "S1"}, {"value": "0.00145459902263464", "module": "C3", "scenario": "S2"}, {"value": "0.000518813956303699", "module": "C4"}, {"value": "-0.000946093310725439", "module": "D", "scenario": "S1"}, {"value": "-0.00607270732256029", "module": "D", "scenario": "S2"}, {"value": "-9.75418665387658E-05", "module": "D", "scenario": "S3"}]}}, {"referenceToLCIAMethodDataSet": {"shortDescription": [{"value": "Bildungspotential für troposphärisches Ozon (POCP)", "lang": "de"}, {"value": "Formation potential of tropospheric ozone photochemical oxidants (POCP)", "lang": "en"}], "type": "LCIA method data set", "refObjectId": "b5c610fe-def3-11e6-bf01-fe55135034f3", "uri": "../lciamethods/b5c610fe-def3-11e6-bf01-fe55135034f3.xml"}, "other": {"anies": [{"name": "referenceToUnitGroupDataSet", "value": {"shortDescription": [{"value": "kg NMVOC-Äq.", "lang": "de"}], "type": "unit group data set", "refObjectId": "d27c25f8-fbc1-44c6-b47b-4adbae4199c6", "uri": "../unitgroups/d27c25f8-fbc1-44c6-b47b-4adbae4199c6.xml"}}, {"value": "0.00118833999942539", "module": "A1-A3"}, {"value": "4.84265883713601E-05", "module": "A4"}, {"value": "1.42348514315762E-05", "module": "A5"}, {"value": "0", "module": "B1"}, {"value": "0.000222973465174724", "module": "B2"}, {"value": "0", "module": "B6"}, {"value": "0", "module": "B7"}, {"value": "8.76467254795489E-06", "module": "C1"}, {"value": "5.62145486746943E-06", "module": "C2"}, {"value": "0.000122253950880167", "module": "C3", "scenario": "S1"}, {"value": "0.000192406543509233", "module": "C3", "scenario": "S2"}, {"value": "0.000150072206357925", "module": "C4"}, {"value": "-0.000312375775512312", "module": "D", "scenario": "S1"}, {"value": "-0.00159149939774181", "module": "D", "scenario": "S2"}, {"value": "-2.56267630592482E-05", "module": "D", "scenario": "S3"}]}}, {"referenceToLCIAMethodDataSet": {"shortDescription": [{"value": "Potenzial für den abiotischen Abbau nicht fossiler Ressourcen (ADPE)", "lang": "de"}, {"value": "Abiotic depletion potential for non fossil resources (ADPE)", "lang": "en"}], "type": "LCIA method data set", "refObjectId": "b2ad6494-c78d-11e6-9d9d-cec0c932ce01", "uri": "../lciamethods/b2ad6494-c78d-11e6-9d9d-cec0c932ce01.xml"}, "other": {"anies": [{"name": "referenceToUnitGroupDataSet", "value": {"shortDescription": [{"value": "kg Sb-Äq.", "lang": "de"}], "type": "unit group data set", "refObjectId": "54ccd2d9-a32a-4fc2-923d-f2c8c93e89d4", "uri": "../unitgroups/54ccd2d9-a32a-4fc2-923d-f2c8c93e89d4.xml"}}, {"value": "4.10187456283183E-07", "module": "A1-A3"}, {"value": "2.9392724239694E-09", "module": "A4"}, {"value": "4.23072104055488E-10", "module": "A5"}, {"value": "0", "module": "B1"}, {"value": "3.212237837681E-09", "module": "B2"}, {"value": "0", "module": "B6"}, {"value": "0", "module": "B7"}, {"value": "8.44492109348854E-11", "module": "C1"}, {"value": "2.84760633585348E-10", "module": "C2"}, {"value": "9.81156397777422E-10", "module": "C3", "scenario": "S1"}, {"value": "1.37787583155086E-09", "module": "C3", "scenario": "S2"}, {"value": "1.81821763142697E-09", "module": "C4"}, {"value": "-2.24379767499063E-08", "module": "D", "scenario": "S1"}, {"value": "-2.52895513319757E-07", "module": "D", "scenario": "S2"}, {"value": "-3.80194390508205E-09", "module": "D", "scenario": "S3"}]}}, {"referenceToLCIAMethodDataSet": {"shortDescription": [{"value": "Potenzial für den abiotischen Abbau fossiler Brennstoffe (ADPF)", "lang": "de"}, {"value": "Abiotic depletion potential for fossil resources (ADPF)", "lang": "en"}], "type": "LCIA method data set", "refObjectId": "b2ad6110-c78d-11e6-9d9d-cec0c932ce01", "uri": "../lciamethods/b2ad6110-c78d-11e6-9d9d-cec0c932ce01.xml"}, "other": {"anies": [{"name": "referenceToUnitGroupDataSet", "value": {"shortDescription": [{"value": "MJ", "lang": "de"}], "type": "unit group data set", "refObjectId": "93a60a57-a3c8-11da-a746-0800200c9a66", "uri": "../unitgroups/93a60a57-a3c8-11da-a746-0800200c9a66.xml"}}, {"value": "18.0708888097551", "module": "A1-A3"}, {"value": "0.552117173326054", "module": "A4"}, {"value": "0.0809790205445063", "module": "A5"}, {"value": "0", "module": "B1"}, {"value": "2.30852839144499", "module": "B2"}, {"value": "0", "module": "B6"}, {"value": "0", "module": "B7"}, {"value": "0.0175255746510594", "module": "C1"}, {"value": "0.0585085411284939", "module": "C2"}, {"value": "1.36826833624149", "module": "C3", "scenario": "S1"}, {"value": "0.372012625752995", "module": "C3", "scenario": "S2"}, {"value": "1.02633143111749", "module": "C4"}, {"value": "-6.70071315877791", "module": "D", "scenario": "S1"}, {"value": "-26.5698797155686", "module": "D", "scenario": "S2"}, {"value": "-0.442997222945105", "module": "D", "scenario": "S3"}]}}, {"referenceToLCIAMethodDataSet": {"shortDescription": [{"value": "Wassernutzung (WDP)", "lang": "de"}, {"value": "Water use (WDP)", "lang": "en"}], "type": "LCIA method data set", "refObjectId": "b2ad66ce-c78d-11e6-9d9d-cec0c932ce01", "uri": "../lciamethods/b2ad66ce-c78d-11e6-9d9d-cec0c932ce01.xml"}, "other": {"anies": [{"name": "referenceToUnitGroupDataSet", "value": {"shortDescription": [{"value": "m^(3) Welt-Äq. entzogen", "lang": "de"}], "type": "unit group data set", "refObjectId": "6ae2df01-888e-46c8-b17d-49fa3869b476", "uri": "../unitgroups/6ae2df01-888e-46c8-b17d-49fa3869b476.xml"}}, {"value": "0.0302112778780379", "module": "A1-A3"}, {"value": "0.000213216521440469", "module": "A4"}, {"value": "0.00882776624766229", "module": "A5"}, {"value": "0", "module": "B1"}, {"value": "0.003183710286881", "module": "B2"}, {"value": "0", "module": "B6"}, {"value": "0", "module": "B7"}, {"value": "1.51771909517884E-05", "module": "C1"}, {"value": "5.18996750146342E-05", "module": "C2"}, {"value": "0.086531390365205", "module": "C3", "scenario": "S1"}, {"value": "0.288657259724133", "module": "C3", "scenario": "S2"}, {"value": "-0.000970592569312617", "module": "C4"}, {"value": "-0.0147262900094822", "module": "D", "scenario": "S1"}, {"value": "-0.114497719463341", "module": "D", "scenario": "S2"}, {"value": "-0.00163881118476761", "module": "D", "scenario": "S3"}]}}, {"referenceToLCIAMethodDataSet": {"shortDescription": [{"value": "Auftreten von Krankheiten aufgrund von Feinstaubemissionen (PM)", "lang": "de"}, {"value": "Incidence of disease due to PM emissions (PM)", "lang": "en"}], "type": "LCIA method data set", "refObjectId": "b5c602c6-def3-11e6-bf01-fe55135034f3", "uri": "../lciamethods/b5c602c6-def3-11e6-bf01-fe55135034f3.xml"}, "other": {"anies": [{"name": "referenceToUnitGroupDataSet", "value": {"shortDescription": [{"value": "Krankheitsfälle", "lang": "de"}], "type": "unit group data set", "refObjectId": "3883559b-648f-4afc-8ba2-0bd24f3affa3", "uri": "../unitgroups/3883559b-648f-4afc-8ba2-0bd24f3affa3.xml"}}, {"value": "2.97051765217853E-08", "module": "A1-A3"}, {"value": "4.47934184708922E-10", "module": "A4"}, {"value": "1.38112876596165E-10", "module": "A5"}, {"value": "0", "module": "B1"}, {"value": "1.45212856290968E-09", "module": "B2"}, {"value": "0", "module": "B6"}, {"value": "0", "module": "B7"}, {"value": "7.5308458219137E-11", "module": "C1"}, {"value": "5.30094285783484E-11", "module": "C2"}, {"value": "1.42658484382027E-09", "module": "C3", "scenario": "S1"}, {"value": "1.8091756408989E-09", "module": "C3", "scenario": "S2"}, {"value": "1.99933264302904E-09", "module": "C4"}, {"value": "-2.34111210639849E-09", "module": "D", "scenario": "S1"}, {"value": "-1.70765024461193E-08", "module": "D", "scenario": "S2"}, {"value": "-2.64650057794538E-10", "module": "D", "scenario": "S3"}]}}, {"referenceToLCIAMethodDataSet": {"shortDescription": [{"value": "Wirkung durch Exposition des Menschen mit U235 (IR)", "lang": "de"}, {"value": "Human exposure efficiency relative to U235 (IR)", "lang": "en"}], "type": "LCIA method data set", "refObjectId": "b5c632be-def3-11e6-bf01-fe55135034f3", "uri": "../lciamethods/b5c632be-def3-11e6-bf01-fe55135034f3.xml"}, "other": {"anies": [{"name": "referenceToUnitGroupDataSet", "value": {"shortDescription": [{"value": "kBq U235-Äq.", "lang": "de"}], "type": "unit group data set", "refObjectId": "456b05bf-1415-44a9-9993-02452f554c09", "uri": "../unitgroups/456b05bf-1415-44a9-9993-02452f554c09.xml"}}, {"value": "0.0255969344174848", "module": "A1-A3"}, {"value": "7.79965429271924E-05", "module": "A4"}, {"value": "8.68373986308474E-05", "module": "A5"}, {"value": "0", "module": "B1"}, {"value": "0.00148637066608862", "module": "B2"}, {"value": "0", "module": "B6"}, {"value": "0", "module": "B7"}, {"value": "4.03951412889931E-06", "module": "C1"}, {"value": "1.63903647437616E-05", "module": "C2"}, {"value": "0.0102473560017423", "module": "C3", "scenario": "S1"}, {"value": "0.00361882697784744", "module": "C3", "scenario": "S2"}, {"value": "0.0017977731349273", "module": "C4"}, {"value": "-0.0235903298935885", "module": "D", "scenario": "S1"}, {"value": "-0.310850551867808", "module": "D", "scenario": "S2"}, {"value": "-0.00444513178868081", "module": "D", "scenario": "S3"}]}}, {"referenceToLCIAMethodDataSet": {"shortDescription": [{"value": "Toxizitätsvergleichseinheit für Ökosysteme (ETP-fw)", "lang": "de"}, {"value": "Comparative toxic unit for ecosystems (ETP-fw)", "lang": "en"}], "type": "LCIA method data set", "refObjectId": "ee1082d1-b0f7-43ca-a1f0-21e2a4a74511", "uri": "../lciamethods/ee1082d1-b0f7-43ca-a1f0-21e2a4a74511.xml"}, "other": {"anies": [{"name": "referenceToUnitGroupDataSet", "value": {"shortDescription": [{"value": "CTUe", "lang": "de"}], "type": "unit group data set", "refObjectId": "aa959ded-f1eb-4efb-9c5c-2d60be36b3e6", "uri": "../unitgroups/aa959ded-f1eb-4efb-9c5c-2d60be36b3e6.xml"}}, {"value": "10.1994138190404", "module": "A1-A3"}, {"value": "0.403067265177675", "module": "A4"}, {"value": "0.0516144297579121", "module": "A5"}, {"value": "0", "module": "B1"}, {"value": "2.60383129555058", "module": "B2"}, {"value": "0", "module": "B6"}, {"value": "0", "module": "B7"}, {"value": "0.0124430301541167", "module": "C1"}, {"value": "0.0419126045096867", "module": "C2"}, {"value": "0.184736492251734", "module": "C3", "scenario": "S1"}, {"value": "0.146189708670706", "module": "C3", "scenario": "S2"}, {"value": "0.87602635018079", "module": "C4"}, {"value": "-2.61520650696293", "module": "D", "scenario": "S1"}, {"value": "-3.65219605869376", "module": "D", "scenario": "S2"}, {"value": "-0.0526994735262543", "module": "D", "scenario": "S3"}]}}, {"referenceToLCIAMethodDataSet": {"shortDescription": [{"value": "Toxizitätsvergleichseinheit für Menschen (krebserregend) (HTP-c)", "lang": "de"}, {"value": "Comparative toxic unit for humans (carcinogenic) (HTP-c)", "lang": "en"}], "type": "LCIA method data set", "refObjectId": "2299222a-bbd8-474f-9d4f-4dd1f18aea7c", "uri": "../lciamethods/2299222a-bbd8-474f-9d4f-4dd1f18aea7c.xml"}, "other": {"anies": [{"name": "referenceToUnitGroupDataSet", "value": {"shortDescription": [{"value": "CTUh", "lang": "de"}], "type": "unit group data set", "refObjectId": "d4c9523e-2d7e-49fd-8469-998f547d3a70", "uri": "../unitgroups/d4c9523e-2d7e-49fd-8469-998f547d3a70.xml"}}, {"value": "3.13776242979718E-10", "module": "A1-A3"}, {"value": "8.03559836092741E-12", "module": "A4"}, {"value": "1.64137809806124E-12", "module": "A5"}, {"value": "0", "module": "B1"}, {"value": "1.5386073064689E-10", "module": "B2"}, {"value": "0", "module": "B6"}, {"value": "0", "module": "B7"}, {"value": "2.51531827214495E-13", "module": "C1"}, {"value": "8.50343477457047E-13", "module": "C2"}, {"value": "9.22225180665421E-12", "module": "C3", "scenario": "S1"}, {"value": "2.03418551703668E-11", "module": "C3", "scenario": "S2"}, {"value": "4.49647671537725E-11", "module": "C4"}, {"value": "-7.37994720913631E-11", "module": "D", "scenario": "S1"}, {"value": "-2.52429179019716E-10", "module": "D", "scenario": "S2"}, {"value": "-4.06682744081482E-12", "module": "D", "scenario": "S3"}]}}, {"referenceToLCIAMethodDataSet": {"shortDescription": [{"value": "Toxizitätsvergleichseinheit für Menschen (nicht krebserregend) (HTP-nc)", "lang": "de"}, {"value": "Comparative toxic unit for humans (noncarcinogenic) (HTP-nc)", "lang": "en"}], "type": "LCIA method data set", "refObjectId": "3af763a5-b7a1-48c9-9cee-1f223481fcef", "uri": "../lciamethods/3af763a5-b7a1-48c9-9cee-1f223481fcef.xml"}, "other": {"anies": [{"name": "referenceToUnitGroupDataSet", "value": {"shortDescription": [{"value": "CTUh", "lang": "de"}], "type": "unit group data set", "refObjectId": "d4c9523e-2d7e-49fd-8469-998f547d3a70", "uri": "../unitgroups/d4c9523e-2d7e-49fd-8469-998f547d3a70.xml"}}, {"value": "7.39441332356105E-09", "module": "A1-A3"}, {"value": "3.36891675557136E-10", "module": "A4"}, {"value": "7.00849942850131E-11", "module": "A5"}, {"value": "0", "module": "B1"}, {"value": "1.24186841772655E-08", "module": "B2"}, {"value": "0", "module": "B6"}, {"value": "0", "module": "B7"}, {"value": "1.11739372646322E-11", "module": "C1"}, {"value": "3.78352101982959E-11", "module": "C2"}, {"value": "3.17730193218457E-10", "module": "C3", "scenario": "S1"}, {"value": "1.52237580200925E-10", "module": "C3", "scenario": "S2"}, {"value": "3.59025642611022E-09", "module": "C4"}, {"value": "-2.60260313238927E-09", "module": "D", "scenario": "S1"}, {"value": "-8.10450682988087E-09", "module": "D", "scenario": "S2"}, {"value": "-1.33927093336875E-10", "module": "D", "scenario": "S3"}]}}, {"referenceToLCIAMethodDataSet": {"shortDescription": [{"value": "Bodenqualitätsindex (SQP)", "lang": "de"}, {"value": "Soil quality index (SQP)", "lang": "en"}], "type": "LCIA method data set", "refObjectId": "b2ad6890-c78d-11e6-9d9d-cec0c932ce01", "uri": "../lciamethods/b2ad6890-c78d-11e6-9d9d-cec0c932ce01.xml"}, "other": {"anies": [{"name": "referenceToUnitGroupDataSet", "value": {"shortDescription": [{"value": "SQP", "lang": "de"}], "type": "unit group data set", "refObjectId": "f130951c-e67f-4f7f-8dd4-665de3974e18", "uri": "../unitgroups/f130951c-e67f-4f7f-8dd4-665de3974e18.xml"}}, {"value": "21.9691336144838", "module": "A1-A3"}, {"value": "0.196538538595839", "module": "A4"}, {"value": "0.0285689842256337", "module": "A5"}, {"value": "0", "module": "B1"}, {"value": "0.101598616670367", "module": "B2"}, {"value": "0", "module": "B6"}, {"value": "0", "module": "B7"}, {"value": "0.0073173807101296", "module": "C1"}, {"value": "0.0244472240995536", "module": "C2"}, {"value": "0.117555932465562", "module": "C3", "scenario": "S1"}, {"value": "0.117270176697498", "module": "C3", "scenario": "S2"}, {"value": "0.0888930415462984", "module": "C4"}, {"value": "-0.423189411244587", "module": "D", "scenario": "S1"}, {"value": "-4.06968370995227", "module": "D", "scenario": "S2"}, {"value": "-0.0582852182486012", "module": "D", "scenario": "S3"}]}}]}, "otherAttributes": {"{http://www.indata.network/EPD/2019}epd-version": "1.2"}, "version": "1.1", "locations": "../ILCDLocations.xml"}