{"processInformation": {"dataSetInformation": {"UUID": "f65e5435-939e-4b4b-8ea7-03f3fba3c290", "name": {"baseName": [{"value": "Flanges and butt welded fittings", "lang": "en"}, {"value": "Flansche und Schweissfittings", "lang": "de"}], "functionalUnitFlowProperties": [{"lang": "en"}]}, "classificationInformation": {"classification": [{"class": [{"value": "Metalle", "level": 0, "classId": "4"}, {"value": "Stahl und Eisen", "level": 1, "classId": "4.1"}, {"value": "Stahlprofile", "level": 2, "classId": "4.1.03"}], "name": "OEKOBAU.DAT"}, {"class": [{"value": "02 Building products", "level": 0}, {"value": "Metallic products and ancillaries", "level": 1}, {"value": "Steel pipes for pressure applications", "level": 2}], "name": "IBUCategories"}]}, "generalComment": [{"value": "This EPD includes the following products depending on application for oil, gas and water pipe systems: \nflanges in carbon steel (also referred to as black steel) or galvanized steel (hot dip galvanized)\nbutt welded fittings in carbon steel (also referred to as black steel) \nThe products covered in this EPD are classified and traded under the following TARif Intgr Communautaire (TARIC) codes: 7307931199, 7307931999, 7307939190, and 7307910090.\nThis EPD specifically excludes the following products:\nproducts in stainless steel\nflange gaskets\n\nthreaded fittings\nvalves.", "lang": "en"}, {"value": "Flansche und stumpfgeschweißte Fittings aus Kohlenstoffstahl oder verzinktem Stahl je nach Anwendung für Öl-, Gas- und Wasserleitungssysteme.", "lang": "de"}]}, "quantitativeReference": {"referenceToReferenceFlow": [0]}, "time": {"referenceYear": 2023, "dataSetValidUntil": 2028, "other": {"anies": [{"name": "publicationDateOfEPD", "value": 1686700800000}]}}, "geography": {"locationOfOperationSupplyOrProduction": {"location": "DK"}}, "technology": {"technologyDescriptionAndIncludedProcesses": [{"value": "The declared products in this EPD are produced from low-alloyed steel, which has been cut, drilled and forged into the shape of a flange or butt weld fitting. Some flanges are hot-dip galvanized. Production happens in China, and then the products are shipped to INDURA in Denmark, where they are mainly sold to the North European market. \nTechnical data: \nFlanges of carbon steel and galvanized steel follow a range of standards in relation to materials, production and technical properties, depending on the type of flanges. The following standards are relevant for Indura's flanges:\nEN1092-1\nASME B16.5\nASME B16.47\nJIS B2220\nEN10025-1\nEN10025-2\nBS EN 10025-2:2019\nEN10222-1\nEN10222-2\nEN10222-4\nEN10028-1\nEN10028-2\nEN10028-6\nDIN 2501\nDIN 2519\nDIN 2527\nDIN 2566\nDIN 2573\nDIN 2576\nDIN 2632\nDIN 2633\nDIN 2634\nDIN 2635\nDIN 2641\nDIN 2642\nDIN 2673\nDIN 28461\nDIN 86030\nDIN 86044\nASTM A105/A105MButt welded fittings of carbon steel follow a range of standards in relation to materials, production and technical properties, depending on the type of fittings. The following standards are relevant for Indura's fittings:\nEN 10253-1\nEN 10253-2\nEN 10217-1\nEN 10217-2\nEN 10217-3\nEN 10217-4\nEN 10216-1\nEN 10216-2\nEN ISO 3183\nASME B16.9\nASTM A234\nDIN 2618\nDIN 2619\nDIN 2642\nDIN 28011 \nDeclared unit: \nThe declared unit is 1 kg of flange or butt welded fitting in carbon steel or galvanized steel, where the highest of each LCIA result is declared on the final EPD.", "lang": "en"}, {"value": "Die in dieser EPD deklarierten Produkte werden aus niedrig legiertem Stahl hergestellt, der in die Form eines Flansches oder Stumpfschweißfittings geschnitten, gebohrt und geschmiedet wurde. Einige Flansche sind feuerverzinkt. Die Produktion findet in China statt, und die Produkte werden dann zu INDURA nach Dänemark verschifft, wo sie hauptsächlich auf dem nordeuropäischen Markt verkauft werden. \nTechnische Daten: \nFlansche aus Kohlenstoffstahl und verzinktem Stahl folgen einer Reihe von Normen in Bezug auf Materialien, Produktion und technische Eigenschaften, je nach Art des Flansches. Die folgenden Normen sind für die Flansche von Indura relevant:EN1092-1ASME B16.5ASME B16.47JIS B2220EN10025-1EN10025-2BS EN 10025-2:2019EN10222-1EN10222-2EN10222-4EN10028-1EN10028-2EN10028-6DIN 2501DIN 2519DIN 2527DIN 2566DIN 2573DIN 2576DIN 2632DIN 2633DIN 2634DIN 2635DIN 2641DIN 2642DIN 2673DIN 28461DIN 86030DIN 86044ASTM A105/A105Mutgeschweißte Fittings aus Kohlenstoffstahl folgen einer Reihe von Normen in Bezug auf die Materialien, Produktion und technische Eigenschaften, je nach Art des Fittings. Die folgenden Normen sind für die Fittings von Indura relevant:EN 10253-1EN 10253-2EN 10217-1EN 10217-2EN 10217-3EN 10217-4EN 10216-1EN 10216-2EN ISO 3183ASME B16.9ASTM A234DIN 2618DIN 2619DIN 2642DIN 28011 \nDeklarierte Einheit: \nDie deklarierte Einheit ist 1 kg Flansch oder stumpfgeschweißter Fitting aus Kohlenstoffstahl oder verzinktem Stahl.", "lang": "de"}], "technologicalApplicability": [{"value": "Flanges and butt welded fittings are used to connect different pipes with each other and can be used both for transporting oils and in connection with water. The flanges are usually in the form of an annular disc and are attached to the end of a pipe, where screws and nuts are used to secure the flange and connect the pipes. The different types of flanges include threaded flanges, blind flanges, welding ring flanges, loose flanges, welding neck flanges, welding neck collars. \n\nButt welded fittings have no threads, which means that they can only be permanently connected by means of a weld. Butt welded fittings cover different types of fittings in various shapes and dimension, such as pipe bends, tees, crosses, welded elbows, saddle elbows, concentric reducers, and excentric reducers.", "lang": "en"}, {"value": "Flansche und stumpfgeschweißte Fittings werden verwendet, um verschiedene Rohre miteinander zu verbinden und können sowohl für den Transport von Ölen als auch in Verbindung mit Wasser verwendet werden. Die Flansche haben in der Regel die Form einer ringförmigen Scheibe und werden am Ende eines Rohres angebracht, wobei Schrauben und Muttern verwendet werden, um den Flansch zu sichern und die Rohre zu verbinden. Zu den verschiedenen Arten von Flanschen gehören Gewindeflansche, Blindflansche, Schweißringflansche, Losflansche, Vorschweißflansche und Vorschweißmuffen. \n\nStumpfgeschweißte Fittings haben kein Gewinde, was bedeutet, dass sie nur durch eine Schweißnaht dauerhaft verbunden werden können. Stumpfgeschweißte Fittings umfassen verschiedene Arten von Fittings in unterschiedlichen Formen und Dimensionen, wie z.B. Rohrbögen, T-Stücke, Kreuze, geschweißte Winkelstücke, Sattelbögen, konzentrische Reduzierstücke und exzentrische Reduzierstücke.", "lang": "de"}]}}, "modellingAndValidation": {"LCIMethodAndAllocation": {"typeOfDataSet": "EPD", "referenceToLCAMethodDetails": [{"shortDescription": [{"value": "Steel pipes for pressure applications.pdf", "lang": "en"}], "type": "source data set", "refObjectId": "76830e29-2e7e-431f-b10a-68003f1a4fa5"}], "other": {"anies": [{"name": "subType", "value": "average dataset"}]}}, "dataSourcesTreatmentAndRepresentativeness": {"referenceToDataSource": [{"shortDescription": [{"value": "ecoinvent database (all versions)", "lang": "en"}], "type": "source data set", "refObjectId": "b497a91f-e14b-4b69-8f28-f50eb1576766"}, {"shortDescription": [{"value": "ecoinvent 3.9 database", "lang": "en"}], "type": "source data set", "refObjectId": "c6825ce7-2951-4e1e-8634-426c7af4679b"}], "useAdviceForDataSet": [{"value": "Scope: \nA life cycle assessment according to ISO 14040/44 has been conducted individually for 1 kg (worst-case product) of the three product groups:\n\nFlanges of carbon steel\nFlanges of galvanized steel\nButt welded fittings of carbon steel\nDue to the variations in products and production locations, the worst-case EPD approach has been applied and the highest environmental impacts have been declared.\n\nThe materials and metal shaping processes originate from a multitude of suppliers which INDURA is not in operational control over. The suppliers' locations are mainly China, but also Vietnam, Cambodia, Slovakia, Romania, and Germany. A conservative average approach has been applied to make the EPD representative for the many suppliers from different locations, thus Chinese and Asian representative data is applied to the calculation in terms of the energy mix and transport distances. INDURAs own facility is located in Vildbjerg, Denmark and emissions from that location are modelled with Danish energy mixes. \nSystem boundary: \nType of EPD: cradle to gate with Modules C1–C4 and Module D.\nThe product stage (modules A1-A3) consists of raw material extraction and processing (A1) as well as the transport to the manufacturing location (A2) and activities at the manufacturing facility (A3). In this study, the processes A1-A3 are all included. Wastes and losses of manufacturing processes are included in the unit processes in which they occur according to the polluter pays principle and the modular approach of EN 15804. Practically this means that the metal scrap is modelled so that its waste processing is included in A3 and credited by reducing the input in A1 to the net consumption of steel. However, this credit cannot exceed the input of secondary metals based on a market average. According to the American Iron and Steel Institute (American Iron and Steel Institute, 2012) the average recycled content of steel is 36.9 % when it originates from basic oxygen furnaces. However, for electric arc furnaces, the recycled content is 89.9 %. The sourced materials from Asia that INDURA purchases are most likely originating from basic oxygen furnaces, but the steel market is constrained (all available ferrous metal is generally recycled). For this reason, a total average of the steel recycled\ncontent should be applied. It is decided that a conservative approach is used in the calculation and the net input of steel is then modelled as primary (virgin) steel.\n\nThe product stages (A1 and A3) for flanges can be seen above.\n\nThe product stages (A1 and A3) for butt welded fittings can be seen above.\n\nAt the end-of-life stage (module C1-C4), INDURAs products are assumed to be manually disassembled from the piping system in which it has been installed. As a result, no processes have been added to the C1 module. Most customers (>93%) are located in Northern Europe (Scandinavia, Germany and Benelux), thus the transportation distances, technology and waste processing will be modelled accordingly. For the waste processing, it is assumed that the product itself will be recycled as metal. 5 % are considered lost during the recycling process and are modelled as inert material landfilling. End-of-life treatment of the packaging is not included in the study. \n\nBenefits and loads beyond the system boundaries (module D) include the potential benefits from reuse, recycling and recovery potentials that are outside the scope of the study. This would include all the flows leaving the product system having passed the end-of-waste stage, thereby allowing the use of them as a substitution for primary material in another product system. Thus, the system will get credit for recycling the collected steel. 5 % are considered lost in the sorting process, thus 95 % of the product is credited in module D.\n\nAs the steel scrap from production processes is credited in the A1-A3 modules, only the end-of-life product will be credited in module D. The scrap should however first reach functional equivalence to steel, which requires it to be processed using an electric arc furnace (EAF) process. The system is then credited with the avoided production of virgin steel produced using the basic oxygen furnace (BOF) process.", "lang": "en"}, {"value": "Gültigkeitsbereich: \nEine Ökobilanz nach ISO 14040/44 wurde individuell für 1 kg der drei Produktgruppen durchgeführt: Flansche aus Kohlenstoffstahl Flansche aus verzinktem Stahl Stumpfgeschweißte Fittings aus KohlenstoffstahlDie Materialien und Metallverarbeitungsprozesse stammen von einer Vielzahl von Lieferanten, über die INDURA keine operative Kontrolle hat. Die Standorte der Lieferanten sind hauptsächlich China, aber auch Vietnam, Kambodscha, die Slowakei, Rumänien und Deutschland. Um die EPD für die vielen Lieferanten aus verschiedenen Standorten repräsentativ zu machen, wurde ein konservativer Durchschnittsansatz angewandt, d.h. für die Berechnung des Energiemixes und der Transportentfernungen wurden repräsentative Daten aus China und Asien verwendet. INDURAs eigene Anlage befindet sich in Vildbjerg, Dänemark, und die Emissionen dieses Standorts wurden mit dem dänischen Energiemix modelliert. Aufgrund der Unterschiede bei den Produkten und Produktionsstandorten wurde der Modell-EPD-Ansatz angewandt und die höchsten Umweltauswirkungen angegeben. \nSystemgrenze: \nArt der EPD: Cradle to Gate mit den Modulen C1-C4 und Modul D. Die Produktstufe (Modul A1-A3) besteht aus der Rohstoffgewinnung und -verarbeitung (A1) sowie dem Transport zum Herstellungsort (A2) und den Aktivitäten in der Herstellungsanlage (A3). In dieser Studie sind die Prozesse A1-A3 alle enthalten. Abfälle und Verluste von Herstellungsprozessen werden gemäß dem Verursacherprinzip und dem modularen Ansatz der EN 15804 in die Einheitsprozesse einbezogen, in denen sie anfallen. In der Praxis bedeutet dies, dass der Metallschrott so modelliert wird, dass seine Abfallverarbeitung in A3 enthalten ist und durch Reduzierung des Inputs in A1 auf den Nettoverbrauch von Stahl angerechnet wird. Diese Gutschrift darf jedoch den Einsatz von Sekundärmetallen auf der Grundlage eines Marktdurchschnitts nicht übersteigen. Nach Angaben des American Iron and Steel Institute (American Iron and Steel Institute, 2012) liegt der durchschnittliche Recyclinganteil von Stahl aus Sauerstoffblasöfen bei 36,9%. Bei Elektrolichtbogenöfen liegt der Recyclinganteil jedoch bei 89,9%. Die von INDURA eingekauften Materialien aus Asien stammen höchstwahrscheinlich aus Sauerstoffblasöfen, aber der Stahlmarkt ist begrenzt (alles verfügbare Eisenmetall wird im Allgemeinen recycelt). Aus diesem Grund sollte ein Gesamtdurchschnitt des recycelten Stahls angesetzt werden. Es wird beschlossen, bei der Berechnung einen konservativen Ansatz zu wählen und den Netto-Stahleinsatz als primären (neuen) Stahl zu modellieren. Die Produktstufen (A1 und A3) für Flansche sind unten zu sehen. Die Produktstufen (A1 und A3) für stumpfgeschweißte Fittings sind unten zu sehen. In der End-of-Life-Phase (Modul C1-C4) wird davon ausgegangen, dass INDURAs Produkte manuell aus dem Rohrleitungssystem, in dem sie installiert wurden, demontiert werden. Aus diesem Grund wurden dem Modul C1 keine Prozesse hinzugefügt. >93% der Kunden befinden sich in Nordeuropa (Skandinavien, Deutschland und Benelux), daher werden die Transportentfernungen, die Technologie und die Abfallverarbeitung entsprechend modelliert. Für die Abfallverarbeitung wird angenommen, dass das Produkt selbst als Metall recycelt wird. Es wird davon ausgegangen, dass 5 % während des Recyclingprozesses verloren gehen und als inertes Material auf der Deponie abgelagert werden. Die End-of-Life-Behandlung der Verpackung ist in der Studie nicht enthalten. \n\nNutzen und Belastungen jenseits der Systemgrenzen (Modul D) umfasst den potenziellen Nutzen aus Wiederverwendungs-, Recycling- und Verwertungspotenzialen, die außerhalb des Rahmens der Studie liegen. Dazu gehören alle Ströme, die das Produktsystem verlassen, nachdem sie das Abfallende überschritten haben, so dass sie als Ersatz für Primärmaterial in einem anderen Produktsystem verwendet werden können. Auf diese Weise erhält das System eine Gutschrift für das Recycling des gesammelten Stahls. Da der Stahlschrott aus den Produktionsprozessen in den Modulen A1-A3 gutgeschrieben wird, wird in Modul D nur das End-of-Life-Produkt gutgeschrieben. Der Schrott muss jedoch zunächst die funktionale Gleichwertigkeit mit Stahl erreichen, was eine Verarbeitung in einem Elektrolichtbogenofen (EAF) erfordert. Dem System wird dann die vermiedene Produktion von neuem Stahl gutgeschrieben, der im Sauerstoff-Basis-Ofen-Verfahren (BOF) hergestellt wurde.", "lang": "de"}], "other": {"anies": [{"name": "referenceToOriginalEPD", "value": {"shortDescription": {"value": "Flanges and butt welded fittings.pdf", "defaultValue": "Flanges and butt welded fittings.pdf", "lstrings": [{"lang": "en", "value": "Flanges and butt welded fittings.pdf"}]}, "type": "source data set", "uuid": {"uuid": "10be6f2a-a487-4fd4-84b1-2b972b513462"}, "refObjectId": "10be6f2a-a487-4fd4-84b1-2b972b513462", "resourceURLs": ["https://oekobaudat.de/OEKOBAU.DAT/resource/sources/10be6f2a-a487-4fd4-84b1-2b972b513462/Flanges_and_butt_welded_fittings_16475.pdf?version=00.01.000"]}}]}}, "validation": {"review": [{"referenceToNameOfReviewerAndInstitution": [{"shortDescription": [{"value": "Institut Bauen und Umwelt e. V.", "lang": "en"}], "type": "contact data set", "refObjectId": "d111dbec-b024-4be5-86c5-752d6eb2cf95", "uri": "../contacts/d111dbec-b024-4be5-86c5-752d6eb2cf95.xml"}], "type": "Accredited third party review"}]}, "complianceDeclarations": {"compliance": [{"referenceToComplianceSystem": {"shortDescription": [{"value": "DIN EN 15804+A2", "lang": "en"}], "type": "source data set", "refObjectId": "c0016b33-8cf7-415c-ac6e-deba0d21440d", "uri": "../sources/c0016b33-8cf7-415c-ac6e-deba0d21440d.xml"}}, {"referenceToComplianceSystem": {"shortDescription": [{"value": "ISO 14025", "lang": "en"}], "type": "source data set", "refObjectId": "4f2eb655-6e44-4874-a95a-e28f5442cd4d", "uri": "../sources/4f2eb655-6e44-4874-a95a-e28f5442cd4d.xml"}}]}}, "administrativeInformation": {"commissionerAndGoal": {"referenceToCommissioner": [{"shortDescription": [{"value": "INDURA", "lang": "en"}], "type": "contact data set", "refObjectId": "cbd57320-e0e8-495a-a504-abeb0a188432", "uri": "../contacts/cbd57320-e0e8-495a-a504-abeb0a188432.xml"}]}, "dataGenerator": {"referenceToPersonOrEntityGeneratingTheDataSet": [{"shortDescription": [{"value": "Viegand Maagøe", "lang": "en"}], "type": "contact data set", "refObjectId": "6ee458a6-649d-4b29-8654-df98d8c74e15", "uri": "../contacts/6ee458a6-649d-4b29-8654-df98d8c74e15.xml"}]}, "dataEntryBy": {"timeStamp": 1686700800000, "referenceToDataSetFormat": [{"shortDescription": [{"value": "ILCD Format", "lang": "en"}], "type": "source data set", "refObjectId": "a97a0155-0234-4b87-b4ce-a45da52f2a40", "uri": "../sources/a97a0155-0234-4b87-b4ce-a45da52f2a40.xml"}, {"shortDescription": [{"value": "EPD-Datenformaterweiterungen v1.2", "lang": "de"}, {"value": "EPD Data Format Extensions v1.2", "lang": "en"}], "type": "source data set", "refObjectId": "a29449fd-aa2f-4de8-b5d7-4b06b43c6fde", "uri": "../sources/a29449fd-aa2f-4de8-b5d7-4b06b43c6fde.xml"}]}, "publicationAndOwnership": {"dataSetVersion": "00.02.000", "referenceToRegistrationAuthority": {"shortDescription": [{"value": "Institut Bauen und Umwelt e. V.", "lang": "en"}], "type": "contact data set", "refObjectId": "d111dbec-b024-4be5-86c5-752d6eb2cf95", "uri": "../contacts/d111dbec-b024-4be5-86c5-752d6eb2cf95.xml"}, "registrationNumber": "EPD-IND-20230122-CBC1-EN", "referenceToOwnershipOfDataSet": {"shortDescription": [{"value": "INDURA", "lang": "en"}], "type": "contact data set", "refObjectId": "cbd57320-e0e8-495a-a504-abeb0a188432", "uri": "../contacts/cbd57320-e0e8-495a-a504-abeb0a188432.xml"}, "copyright": true, "licenseType": "Free of charge for all users and uses", "accessRestrictions": [{"value": "None", "lang": "en"}], "other": {"anies": [{"name": "referenceToPublisher", "value": {"shortDescription": [{"value": "Institut Bauen und Umwelt e. V.", "lang": "en"}], "type": "contact data set", "refObjectId": "d111dbec-b024-4be5-86c5-752d6eb2cf95", "uri": "../contacts/d111dbec-b024-4be5-86c5-752d6eb2cf95.xml"}}]}}}, "exchanges": {"exchange": [{"dataSetInternalID": 0, "referenceToFlowDataSet": {"shortDescription": [{"value": "1 kg of flange or butt welded fitting of carbon steel or galvanised steel (Flansche und stumpfgeschweißte Fittings aus Kohlenstoffstahl oder verzinktem Stahl je nach Anwendung für Öl-, Gas- und Wasserleitungssysteme.)", "lang": "en"}], "type": "flow data set", "refObjectId": "8c23e412-53e7-dd2e-a03b-515194390c4d", "uri": "../flows/8c23e412-53e7-dd2e-a03b-515194390c4d.xml"}, "meanAmount": 1.0, "referencesToDataSource": {}, "referenceFlow": true, "resolvedFlowVersion": "00.02.000", "resultingflowAmount": 1.0, "flowProperties": [{"name": [{"lang": "en", "value": "Mass"}, {"lang": "de", "value": "Masse"}], "uuid": "93a60a56-a3c8-11da-a746-0800200b9a66", "referenceFlowProperty": true, "meanValue": 1.0, "referenceUnit": "kg", "unitGroupUUID": "ad38d542-3fe9-439d-9b95-2f5f7752acaf"}], "typeOfFlow": "Product flow", "classification": {"classHierarchy": "Metalle / Stahl und Eisen / Stahlprofile", "name": "OEKOBAU.DAT"}}, {"dataSetInternalID": 1, "referenceToFlowDataSet": {"shortDescription": [{"value": "Renewable primary energy as energy carrier (PERE)", "lang": "en"}, {"value": "Erneuerbare Primärenergie als Energieträger (PERE)", "lang": "de"}], "type": "flow data set", "refObjectId": "20f32be5-0398-4288-9b6d-accddd195317", "uri": "../flows/20f32be5-0398-4288-9b6d-accddd195317.xml"}, "exchange direction": "INPUT", "other": {"anies": [{"name": "referenceToUnitGroupDataSet", "value": {"shortDescription": [{"value": "MJ", "lang": "en"}], "type": "unit group data set", "refObjectId": "93a60a57-a3c8-11da-a746-0800200c9a66", "uri": "../unitgroups/93a60a57-a3c8-11da-a746-0800200c9a66.xml"}}, {"value": "5.0034258037548", "module": "A1-A3"}, {"value": "0", "module": "C1"}, {"value": "0.000953218584920376", "module": "C2"}, {"value": "0.0536108058388126", "module": "C3"}, {"value": "6.4788760823001E-05", "module": "C4"}, {"value": "-0.714889773623072", "module": "D"}]}, "resolvedFlowVersion": "38.00.000", "flowProperties": [], "typeOfFlow": "Other flow", "classification": {"classHierarchy": "Quantities", "name": "GaBiCategories"}}, {"dataSetInternalID": 2, "referenceToFlowDataSet": {"shortDescription": [{"value": "Renewable primary energy resources as material utilization (PERM)", "lang": "en"}, {"value": "Erneuerbare Primärenergie zur stofflichen Nutzung (PERM)", "lang": "de"}], "type": "flow data set", "refObjectId": "fb3ec0de-548d-4508-aea5-00b73bf6f702", "uri": "../flows/fb3ec0de-548d-4508-aea5-00b73bf6f702.xml"}, "exchange direction": "INPUT", "other": {"anies": [{"name": "referenceToUnitGroupDataSet", "value": {"shortDescription": [{"value": "MJ", "lang": "en"}], "type": "unit group data set", "refObjectId": "93a60a57-a3c8-11da-a746-0800200c9a66", "uri": "../unitgroups/93a60a57-a3c8-11da-a746-0800200c9a66.xml"}}, {"value": "2.16530507619129", "module": "A1-A3"}, {"value": "0", "module": "C1"}, {"value": "0", "module": "C2"}, {"value": "0", "module": "C3"}, {"value": "0", "module": "C4"}, {"value": "0", "module": "D"}]}, "resolvedFlowVersion": "38.00.000", "flowProperties": [], "typeOfFlow": "Other flow", "classification": {"classHierarchy": "Quantities", "name": "GaBiCategories"}}, {"dataSetInternalID": 3, "referenceToFlowDataSet": {"shortDescription": [{"value": "Total use of renewable primary energy resources (PERT)", "lang": "en"}, {"value": "Total erneuerbare Primärenergie (PERT)", "lang": "de"}], "type": "flow data set", "refObjectId": "53f97275-fa8a-4cdd-9024-65936002acd0", "uri": "../flows/53f97275-fa8a-4cdd-9024-65936002acd0.xml"}, "exchange direction": "INPUT", "other": {"anies": [{"name": "referenceToUnitGroupDataSet", "value": {"shortDescription": [{"value": "MJ", "lang": "en"}], "type": "unit group data set", "refObjectId": "93a60a57-a3c8-11da-a746-0800200c9a66", "uri": "../unitgroups/93a60a57-a3c8-11da-a746-0800200c9a66.xml"}}, {"value": "7.16873087994609", "module": "A1-A3"}, {"value": "0", "module": "C1"}, {"value": "0.000953218584920376", "module": "C2"}, {"value": "0.0536108058388126", "module": "C3"}, {"value": "6.4788760823001E-05", "module": "C4"}, {"value": "-0.714889773623072", "module": "D"}]}, "resolvedFlowVersion": "38.00.000", "flowProperties": [], "typeOfFlow": "Other flow", "classification": {"classHierarchy": "Quantities / Environmental quantities / EPD EN 15804 / LCI indicators", "name": "GaBiCategories"}}, {"dataSetInternalID": 4, "referenceToFlowDataSet": {"shortDescription": [{"value": "Non renewable primary energy as energy carrier (PENRE)", "lang": "en"}, {"value": "Nicht-erneuerbare Primärenergie als Energieträger (PENRE)", "lang": "de"}], "type": "flow data set", "refObjectId": "ac857178-2b45-46ec-892a-a9a4332f0372", "uri": "../flows/ac857178-2b45-46ec-892a-a9a4332f0372.xml"}, "exchange direction": "INPUT", "other": {"anies": [{"name": "referenceToUnitGroupDataSet", "value": {"shortDescription": [{"value": "MJ", "lang": "en"}], "type": "unit group data set", "refObjectId": "93a60a57-a3c8-11da-a746-0800200c9a66", "uri": "../unitgroups/93a60a57-a3c8-11da-a746-0800200c9a66.xml"}}, {"value": "65.4725929240983", "module": "A1-A3"}, {"value": "0", "module": "C1"}, {"value": "0.060724612053621", "module": "C2"}, {"value": "0.3068029510396", "module": "C3"}, {"value": "0.00771436621649718", "module": "C4"}, {"value": "-10.3352675102822", "module": "D"}]}, "resolvedFlowVersion": "38.00.000", "flowProperties": [], "typeOfFlow": "Other flow", "classification": {"classHierarchy": "Quantities", "name": "GaBiCategories"}}, {"dataSetInternalID": 5, "referenceToFlowDataSet": {"shortDescription": [{"value": "Non renewable primary energy as material utilization (PENRM)", "lang": "en"}, {"value": "Nicht-erneuerbare Primärenergie zur stofflichen Nutzung (PENRM)", "lang": "de"}], "type": "flow data set", "refObjectId": "1421caa0-679d-4bf4-b282-0eb850ccae27", "uri": "../flows/1421caa0-679d-4bf4-b282-0eb850ccae27.xml"}, "exchange direction": "INPUT", "other": {"anies": [{"name": "referenceToUnitGroupDataSet", "value": {"shortDescription": [{"value": "MJ", "lang": "en"}], "type": "unit group data set", "refObjectId": "93a60a57-a3c8-11da-a746-0800200c9a66", "uri": "../unitgroups/93a60a57-a3c8-11da-a746-0800200c9a66.xml"}}, {"value": "0.328376390475374", "module": "A1-A3"}, {"value": "0", "module": "C1"}, {"value": "0", "module": "C2"}, {"value": "0", "module": "C3"}, {"value": "0", "module": "C4"}, {"value": "0", "module": "D"}]}, "resolvedFlowVersion": "38.00.000", "flowProperties": [], "typeOfFlow": "Other flow", "classification": {"classHierarchy": "Quantities", "name": "GaBiCategories"}}, {"dataSetInternalID": 6, "referenceToFlowDataSet": {"shortDescription": [{"value": "Total use of non renewable primary energy resources (PENRT)", "lang": "en"}, {"value": "Total nicht erneuerbare Primärenergie (PENRT)", "lang": "de"}], "type": "flow data set", "refObjectId": "06159210-646b-4c8d-8583-da9b3b95a6c1", "uri": "../flows/06159210-646b-4c8d-8583-da9b3b95a6c1.xml"}, "exchange direction": "INPUT", "other": {"anies": [{"name": "referenceToUnitGroupDataSet", "value": {"shortDescription": [{"value": "MJ", "lang": "en"}], "type": "unit group data set", "refObjectId": "93a60a57-a3c8-11da-a746-0800200c9a66", "uri": "../unitgroups/93a60a57-a3c8-11da-a746-0800200c9a66.xml"}}, {"value": "65.8009693145737", "module": "A1-A3"}, {"value": "0", "module": "C1"}, {"value": "0.060724612053621", "module": "C2"}, {"value": "0.3068029510396", "module": "C3"}, {"value": "0.00771436621649718", "module": "C4"}, {"value": "-10.3352675102822", "module": "D"}]}, "resolvedFlowVersion": "38.00.000", "flowProperties": [], "typeOfFlow": "Other flow", "classification": {"classHierarchy": "Quantities / Environmental quantities / EPD EN 15804 / LCI indicators", "name": "GaBiCategories"}}, {"dataSetInternalID": 7, "referenceToFlowDataSet": {"shortDescription": [{"value": "Use of secondary material (SM)", "lang": "en"}, {"value": "Einsatz von Sekundärstoffen (SM)", "lang": "de"}], "type": "flow data set", "refObjectId": "c6a1f35f-2d09-4f54-8dfb-97e502e1ce92", "uri": "../flows/c6a1f35f-2d09-4f54-8dfb-97e502e1ce92.xml"}, "exchange direction": "INPUT", "other": {"anies": [{"name": "referenceToUnitGroupDataSet", "value": {"shortDescription": [{"value": "kg", "lang": "en"}], "type": "unit group data set", "refObjectId": "ad38d542-3fe9-439d-9b95-2f5f7752acaf", "uri": "../unitgroups/ad38d542-3fe9-439d-9b95-2f5f7752acaf.xml"}}, {"value": "0.796283325099228", "module": "A1-A3"}, {"value": "0", "module": "C1"}, {"value": "2.70490622142766E-05", "module": "C2"}, {"value": "0.000341803097188744", "module": "C3"}, {"value": "1.85932124776841E-06", "module": "C4"}, {"value": "0.781672980728968", "module": "D"}]}, "resolvedFlowVersion": "38.00.000", "flowProperties": [], "typeOfFlow": "Other flow", "classification": {"classHierarchy": "Quantities / Environmental quantities / EPD EN 15804 / LCI indicators", "name": "GaBiCategories"}}, {"dataSetInternalID": 8, "referenceToFlowDataSet": {"shortDescription": [{"value": "Use of renewable secondary fuels (RSF)", "lang": "en"}, {"value": "Erneuerbare Sekundärbrennstoffe (RSF)", "lang": "de"}], "type": "flow data set", "refObjectId": "64333088-a55f-4aa2-9a31-c10b07816787", "uri": "../flows/64333088-a55f-4aa2-9a31-c10b07816787.xml"}, "exchange direction": "INPUT", "other": {"anies": [{"name": "referenceToUnitGroupDataSet", "value": {"shortDescription": [{"value": "MJ", "lang": "en"}], "type": "unit group data set", "refObjectId": "93a60a57-a3c8-11da-a746-0800200c9a66", "uri": "../unitgroups/93a60a57-a3c8-11da-a746-0800200c9a66.xml"}}, {"value": "0.017459764070599", "module": "A1-A3"}, {"value": "0", "module": "C1"}, {"value": "3.3365205982554E-07", "module": "C2"}, {"value": "1.7198235039946E-05", "module": "C3"}, {"value": "3.98655729405729E-08", "module": "C4"}, {"value": "-8.44251459840375E-05", "module": "D"}]}, "resolvedFlowVersion": "38.00.000", "flowProperties": [], "typeOfFlow": "Other flow", "classification": {"classHierarchy": "Quantities / Environmental quantities / EPD EN 15804 / LCI indicators", "name": "GaBiCategories"}}, {"dataSetInternalID": 9, "referenceToFlowDataSet": {"shortDescription": [{"value": "Use of non renewable secondary fuels (NRSF)", "lang": "en"}, {"value": "Nicht erneuerbare Sekundärbrennstoffe (NRSF)", "lang": "de"}], "type": "flow data set", "refObjectId": "89def144-d39a-4287-b86f-efde453ddcb2", "uri": "../flows/89def144-d39a-4287-b86f-efde453ddcb2.xml"}, "exchange direction": "INPUT", "other": {"anies": [{"name": "referenceToUnitGroupDataSet", "value": {"shortDescription": [{"value": "MJ", "lang": "en"}], "type": "unit group data set", "refObjectId": "93a60a57-a3c8-11da-a746-0800200c9a66", "uri": "../unitgroups/93a60a57-a3c8-11da-a746-0800200c9a66.xml"}}, {"value": "0", "module": "A1-A3"}, {"value": "0", "module": "C1"}, {"value": "0", "module": "C2"}, {"value": "0", "module": "C3"}, {"value": "0", "module": "C4"}, {"value": "0", "module": "D"}]}, "resolvedFlowVersion": "38.00.000", "flowProperties": [], "typeOfFlow": "Other flow", "classification": {"classHierarchy": "Quantities / Environmental quantities / EPD EN 15804 / LCI indicators", "name": "GaBiCategories"}}, {"dataSetInternalID": 10, "referenceToFlowDataSet": {"shortDescription": [{"value": "Use of net fresh water (FW)", "lang": "en"}, {"value": "Einsatz von Süßwasserressourcen (FW)", "lang": "de"}], "type": "flow data set", "refObjectId": "3cf952c8-f3a4-461d-8c96-96456ca62246", "uri": "../flows/3cf952c8-f3a4-461d-8c96-96456ca62246.xml"}, "exchange direction": "INPUT", "other": {"anies": [{"name": "referenceToUnitGroupDataSet", "value": {"shortDescription": [{"value": "m^3", "lang": "en"}], "type": "unit group data set", "refObjectId": "cd950537-0a98-4044-9ba7-9f9a68d0a504", "uri": "../unitgroups/cd950537-0a98-4044-9ba7-9f9a68d0a504.xml"}}, {"value": "0.0231541993696346", "module": "A1-A3"}, {"value": "0", "module": "C1"}, {"value": "7.72540003357128E-06", "module": "C2"}, {"value": "0.000155502112701554", "module": "C3"}, {"value": "7.97105144740953E-06", "module": "C4"}, {"value": "-0.00201424908856112", "module": "D"}]}, "resolvedFlowVersion": "38.00.000", "flowProperties": [], "typeOfFlow": "Other flow", "classification": {"classHierarchy": "Quantities / Environmental quantities / EPD EN 15804 / LCI indicators", "name": "GaBiCategories"}}, {"dataSetInternalID": 11, "referenceToFlowDataSet": {"shortDescription": [{"value": "Hazardous waste disposed (HWD)", "lang": "en"}, {"value": "Gefährlicher Abfall zur Deponie (HWD)", "lang": "de"}], "type": "flow data set", "refObjectId": "430f9e0f-59b2-46a0-8e0d-55e0e84948fc", "uri": "../flows/430f9e0f-59b2-46a0-8e0d-55e0e84948fc.xml"}, "exchange direction": "OUTPUT", "other": {"anies": [{"name": "referenceToUnitGroupDataSet", "value": {"shortDescription": [{"value": "kg", "lang": "en"}], "type": "unit group data set", "refObjectId": "ad38d542-3fe9-439d-9b95-2f5f7752acaf", "uri": "../unitgroups/ad38d542-3fe9-439d-9b95-2f5f7752acaf.xml"}}, {"value": "0.623463088373505", "module": "A1-A3"}, {"value": "0", "module": "C1"}, {"value": "4.07913669172278E-05", "module": "C2"}, {"value": "0.00082351632783633", "module": "C3"}, {"value": "3.70360073757284E-06", "module": "C4"}, {"value": "-0.16351672975657", "module": "D"}]}, "resolvedFlowVersion": "38.00.000", "flowProperties": [], "typeOfFlow": "Other flow", "classification": {"classHierarchy": "Quantities / Environmental quantities / EPD EN 15804 / LCI indicators", "name": "GaBiCategories"}}, {"dataSetInternalID": 12, "referenceToFlowDataSet": {"shortDescription": [{"value": "Non hazardous waste disposed (NHWD)", "lang": "en"}, {"value": "Entsorgter nicht gefährlicher Abfall (NHWD)", "lang": "de"}], "type": "flow data set", "refObjectId": "b29ef66b-e286-4afa-949f-62f1a7b4d7fa", "uri": "../flows/b29ef66b-e286-4afa-949f-62f1a7b4d7fa.xml"}, "exchange direction": "OUTPUT", "other": {"anies": [{"name": "referenceToUnitGroupDataSet", "value": {"shortDescription": [{"value": "kg", "lang": "en"}], "type": "unit group data set", "refObjectId": "ad38d542-3fe9-439d-9b95-2f5f7752acaf", "uri": "../unitgroups/ad38d542-3fe9-439d-9b95-2f5f7752acaf.xml"}}, {"value": "8.03879277499708", "module": "A1-A3"}, {"value": "0", "module": "C1"}, {"value": "0.0012713129085978", "module": "C2"}, {"value": "0.0584634449480939", "module": "C3"}, {"value": "0.000110801872113459", "module": "C4"}, {"value": "-1.9764454299678", "module": "D"}]}, "resolvedFlowVersion": "38.00.000", "flowProperties": [], "typeOfFlow": "Other flow", "classification": {"classHierarchy": "Quantities / Environmental quantities / EPD EN 15804 / LCI indicators", "name": "GaBiCategories"}}, {"dataSetInternalID": 13, "referenceToFlowDataSet": {"shortDescription": [{"value": "Radioactive waste disposed (RWD)", "lang": "en"}, {"value": "Entsorgter radioaktiver Abfall (RWD)", "lang": "de"}], "type": "flow data set", "refObjectId": "3449546e-52ad-4b39-b809-9fb77cea8ff6", "uri": "../flows/3449546e-52ad-4b39-b809-9fb77cea8ff6.xml"}, "exchange direction": "OUTPUT", "other": {"anies": [{"name": "referenceToUnitGroupDataSet", "value": {"shortDescription": [{"value": "kg", "lang": "en"}], "type": "unit group data set", "refObjectId": "ad38d542-3fe9-439d-9b95-2f5f7752acaf", "uri": "../unitgroups/ad38d542-3fe9-439d-9b95-2f5f7752acaf.xml"}}, {"value": "1.77014066725096E-05", "module": "A1-A3"}, {"value": "0", "module": "C1"}, {"value": "4.97401717174083E-09", "module": "C2"}, {"value": "1.6641719175567E-07", "module": "C3"}, {"value": "3.24029629582034E-10", "module": "C4"}, {"value": "2.48936058521722E-06", "module": "D"}]}, "resolvedFlowVersion": "38.00.000", "flowProperties": [], "typeOfFlow": "Other flow", "classification": {"classHierarchy": "Quantities / Environmental quantities / EPD EN 15804 / LCI indicators", "name": "GaBiCategories"}}, {"dataSetInternalID": 14, "referenceToFlowDataSet": {"shortDescription": [{"value": "Components for re-use (CRU)", "lang": "en"}, {"value": "Komponenten für die Wiederverwendung (CRU)", "lang": "de"}], "type": "flow data set", "refObjectId": "a2b32f97-3fc7-4af2-b209-525bc6426f33", "uri": "../flows/a2b32f97-3fc7-4af2-b209-525bc6426f33.xml"}, "exchange direction": "OUTPUT", "other": {"anies": [{"name": "referenceToUnitGroupDataSet", "value": {"shortDescription": [{"value": "kg", "lang": "en"}], "type": "unit group data set", "refObjectId": "ad38d542-3fe9-439d-9b95-2f5f7752acaf", "uri": "../unitgroups/ad38d542-3fe9-439d-9b95-2f5f7752acaf.xml"}}, {"value": "0", "module": "A1-A3"}, {"value": "0", "module": "C1"}, {"value": "0", "module": "C2"}, {"value": "0", "module": "C3"}, {"value": "0", "module": "C4"}, {"value": "0", "module": "D"}]}, "resolvedFlowVersion": "38.00.000", "flowProperties": [], "typeOfFlow": "Other flow", "classification": {"classHierarchy": "Quantities / Environmental quantities / EPD EN 15804 / LCI indicators", "name": "GaBiCategories"}}, {"dataSetInternalID": 15, "referenceToFlowDataSet": {"shortDescription": [{"value": "Materials for recycling (MFR)", "lang": "en"}, {"value": "Stoffe zum Recycling (MFR)", "lang": "de"}], "type": "flow data set", "refObjectId": "d7fe48a5-4103-49c8-9aae-b0b5dfdbd6ae", "uri": "../flows/d7fe48a5-4103-49c8-9aae-b0b5dfdbd6ae.xml"}, "exchange direction": "OUTPUT", "other": {"anies": [{"name": "referenceToUnitGroupDataSet", "value": {"shortDescription": [{"value": "kg", "lang": "en"}], "type": "unit group data set", "refObjectId": "ad38d542-3fe9-439d-9b95-2f5f7752acaf", "uri": "../unitgroups/ad38d542-3fe9-439d-9b95-2f5f7752acaf.xml"}}, {"value": "0.513504325982816", "module": "A1-A3"}, {"value": "0", "module": "C1"}, {"value": "4.57359130512097E-07", "module": "C2"}, {"value": "1.00001319727716", "module": "C3"}, {"value": "3.45562420064479E-08", "module": "C4"}, {"value": "-6.79435353116422E-05", "module": "D"}]}, "resolvedFlowVersion": "38.00.000", "flowProperties": [], "typeOfFlow": "Other flow", "classification": {"classHierarchy": "Quantities / Environmental quantities / EPD EN 15804 / LCI indicators", "name": "GaBiCategories"}}, {"dataSetInternalID": 16, "referenceToFlowDataSet": {"shortDescription": [{"value": "Materials for energy recovery (MER)", "lang": "en"}, {"value": "Stoffe für die Energierückgewinnung (MER)", "lang": "de"}], "type": "flow data set", "refObjectId": "59a9181c-3aaf-46ee-8b13-2b3723b6e447", "uri": "../flows/59a9181c-3aaf-46ee-8b13-2b3723b6e447.xml"}, "exchange direction": "OUTPUT", "other": {"anies": [{"name": "referenceToUnitGroupDataSet", "value": {"shortDescription": [{"value": "kg", "lang": "en"}], "type": "unit group data set", "refObjectId": "ad38d542-3fe9-439d-9b95-2f5f7752acaf", "uri": "../unitgroups/ad38d542-3fe9-439d-9b95-2f5f7752acaf.xml"}}, {"value": "5.55714265698809E-05", "module": "A1-A3"}, {"value": "0", "module": "C1"}, {"value": "2.81527887085966E-09", "module": "C2"}, {"value": "4.6329613387736E-08", "module": "C3"}, {"value": "1.24336542374701E-10", "module": "C4"}, {"value": "-5.94669961837962E-06", "module": "D"}]}, "resolvedFlowVersion": "38.00.000", "flowProperties": [], "typeOfFlow": "Other flow", "classification": {"classHierarchy": "Quantities / Environmental quantities / EPD EN 15804 / LCI indicators", "name": "GaBiCategories"}}, {"dataSetInternalID": 17, "referenceToFlowDataSet": {"shortDescription": [{"value": "Exported electrical energy (EEE)", "lang": "en"}, {"value": "Exportierte elektrische Energie (EEE)", "lang": "de"}], "type": "flow data set", "refObjectId": "4da0c987-2b76-40d6-9e9e-82a017aaaf29", "uri": "../flows/4da0c987-2b76-40d6-9e9e-82a017aaaf29.xml"}, "exchange direction": "OUTPUT", "other": {"anies": [{"name": "referenceToUnitGroupDataSet", "value": {"shortDescription": [{"value": "MJ", "lang": "en"}], "type": "unit group data set", "refObjectId": "93a60a57-a3c8-11da-a746-0800200c9a66", "uri": "../unitgroups/93a60a57-a3c8-11da-a746-0800200c9a66.xml"}}, {"value": "0.0213176001606592", "module": "A1-A3"}, {"value": "0", "module": "C1"}, {"value": "1.00048237126671E-05", "module": "C2"}, {"value": "0.000375470724602928", "module": "C3"}, {"value": "4.23837390856352E-07", "module": "C4"}, {"value": "0.0111267212123633", "module": "D"}]}, "resolvedFlowVersion": "38.00.000", "flowProperties": [], "typeOfFlow": "Other flow", "classification": {"classHierarchy": "Quantities / Environmental quantities / EPD EN 15804 / LCI indicators", "name": "GaBiCategories"}}, {"dataSetInternalID": 18, "referenceToFlowDataSet": {"shortDescription": [{"value": "Exported thermal energy (EET)", "lang": "en"}, {"value": "Exportierte thermische Energie (EET)", "lang": "de"}], "type": "flow data set", "refObjectId": "98daf38a-7a79-46d3-9a37-2b7bd0955810", "uri": "../flows/98daf38a-7a79-46d3-9a37-2b7bd0955810.xml"}, "exchange direction": "OUTPUT", "other": {"anies": [{"name": "referenceToUnitGroupDataSet", "value": {"shortDescription": [{"value": "MJ", "lang": "en"}], "type": "unit group data set", "refObjectId": "93a60a57-a3c8-11da-a746-0800200c9a66", "uri": "../unitgroups/93a60a57-a3c8-11da-a746-0800200c9a66.xml"}}, {"value": "0.026444441804627", "module": "A1-A3"}, {"value": "0", "module": "C1"}, {"value": "2.37456131858319E-05", "module": "C2"}, {"value": "5.75747872655514E-05", "module": "C3"}, {"value": "2.6403954849908E-07", "module": "C4"}, {"value": "-0.00960413760482631", "module": "D"}]}, "resolvedFlowVersion": "38.00.000", "flowProperties": [], "typeOfFlow": "Other flow", "classification": {"classHierarchy": "Quantities / Environmental quantities / EPD EN 15804 / LCI indicators", "name": "GaBiCategories"}}]}, "LCIAResults": {"LCIAResult": [{"referenceToLCIAMethodDataSet": {"shortDescription": [{"value": "Global Warming Potential total (GWP-total)", "lang": "en"}, {"value": "Globales Erwärmungspotenzial total (GWP-total)", "lang": "de"}], "type": "LCIA method data set", "refObjectId": "6a37f984-a4b3-458a-a20a-64418c145fa2", "uri": "../lciamethods/6a37f984-a4b3-458a-a20a-64418c145fa2.xml"}, "other": {"anies": [{"name": "referenceToUnitGroupDataSet", "value": {"shortDescription": [{"value": "kg CO_(2) eq", "lang": "en"}], "type": "unit group data set", "refObjectId": "1ebf3012-d0db-4de2-aefd-ef30cedb0be1", "uri": "../unitgroups/1ebf3012-d0db-4de2-aefd-ef30cedb0be1.xml"}}, {"value": "5.68714597758194", "module": "A1-A3"}, {"value": "0", "module": "C1"}, {"value": "0.00418052607873165", "module": "C2"}, {"value": "0.0220610193978529", "module": "C3"}, {"value": "0.0003076085515812", "module": "C4"}, {"value": "-1.10892133420341", "module": "D"}]}}, {"referenceToLCIAMethodDataSet": {"shortDescription": [{"value": "Global Warming Potential fossil fuels (GWP-fossil)", "lang": "en"}, {"value": "Globales Erwärmungspotenzial fossil (GWP-fossil)", "lang": "de"}], "type": "LCIA method data set", "refObjectId": "5f635281-343e-44fb-83df-1971b155e6b6", "uri": "../lciamethods/5f635281-343e-44fb-83df-1971b155e6b6.xml"}, "other": {"anies": [{"name": "referenceToUnitGroupDataSet", "value": {"shortDescription": [{"value": "kg CO_(2) eq", "lang": "en"}], "type": "unit group data set", "refObjectId": "1ebf3012-d0db-4de2-aefd-ef30cedb0be1", "uri": "../unitgroups/1ebf3012-d0db-4de2-aefd-ef30cedb0be1.xml"}}, {"value": "5.66089749175674", "module": "A1-A3"}, {"value": "0", "module": "C1"}, {"value": "0.00417517309149854", "module": "C2"}, {"value": "0.0224978271638976", "module": "C3"}, {"value": "0.00030726178375619", "module": "C4"}, {"value": "-1.11177362090324", "module": "D"}]}}, {"referenceToLCIAMethodDataSet": {"shortDescription": [{"value": "Global Warming Potential biogenic (GWP-biogenic)", "lang": "en"}, {"value": "Globales Erwärmungspotenzial biogen (GWP-biogenic)", "lang": "de"}], "type": "LCIA method data set", "refObjectId": "2356e1ab-0185-4db5-86e5-16de51c7485c", "uri": "../lciamethods/2356e1ab-0185-4db5-86e5-16de51c7485c.xml"}, "other": {"anies": [{"name": "referenceToUnitGroupDataSet", "value": {"shortDescription": [{"value": "kg CO_(2) eq", "lang": "en"}], "type": "unit group data set", "refObjectId": "1ebf3012-d0db-4de2-aefd-ef30cedb0be1", "uri": "../unitgroups/1ebf3012-d0db-4de2-aefd-ef30cedb0be1.xml"}}, {"value": "0.0202688803392823", "module": "A1-A3"}, {"value": "0", "module": "C1"}, {"value": "3.31195121322697E-06", "module": "C2"}, {"value": "-0.000464045518167515", "module": "C3"}, {"value": "1.61244868499824E-07", "module": "C4"}, {"value": "0.00435633968068091", "module": "D"}]}}, {"referenceToLCIAMethodDataSet": {"shortDescription": [{"value": "Global Warming Potential luluc (GWP-luluc)", "lang": "en"}, {"value": "Globales Erwärmungspotenzial luluc (GWP-luluc)", "lang": "de"}], "type": "LCIA method data set", "refObjectId": "4331bbdb-978a-490d-8707-eeb047f01a55", "uri": "../lciamethods/4331bbdb-978a-490d-8707-eeb047f01a55.xml"}, "other": {"anies": [{"name": "referenceToUnitGroupDataSet", "value": {"shortDescription": [{"value": "kg CO_(2) eq", "lang": "en"}], "type": "unit group data set", "refObjectId": "1ebf3012-d0db-4de2-aefd-ef30cedb0be1", "uri": "../unitgroups/1ebf3012-d0db-4de2-aefd-ef30cedb0be1.xml"}}, {"value": "0.0146702690336997", "module": "A1-A3"}, {"value": "0", "module": "C1"}, {"value": "2.04103601988158E-06", "module": "C2"}, {"value": "2.72377521228482E-05", "module": "C3"}, {"value": "1.85522956509644E-07", "module": "C4"}, {"value": "-0.000205863756007115", "module": "D"}]}}, {"referenceToLCIAMethodDataSet": {"shortDescription": [{"value": "Depletion potential of the stratospheric ozone layer (ODP)", "lang": "en"}, {"value": "Abbau Potential der stratosphärischen Ozonschicht (ODP)", "lang": "de"}], "type": "LCIA method data set", "refObjectId": "b5c629d6-def3-11e6-bf01-fe55135034f3", "uri": "../lciamethods/b5c629d6-def3-11e6-bf01-fe55135034f3.xml"}, "other": {"anies": [{"name": "referenceToUnitGroupDataSet", "value": {"shortDescription": [{"value": "kg CFC11 eq", "lang": "en"}], "type": "unit group data set", "refObjectId": "d9e957c9-7309-4474-bf3a-7777df6c4e5b", "uri": "../unitgroups/d9e957c9-7309-4474-bf3a-7777df6c4e5b.xml"}}, {"value": "9.66791388492761E-08", "module": "A1-A3"}, {"value": "0", "module": "C1"}, {"value": "9.16133902275552E-11", "module": "C2"}, {"value": "3.54404926980317E-10", "module": "C3"}, {"value": "8.89807339335647E-12", "module": "C4"}, {"value": "-2.40498537304161E-08", "module": "D"}]}}, {"referenceToLCIAMethodDataSet": {"shortDescription": [{"value": "Acidification potential of land and water (AP)", "lang": "en"}, {"value": "Versauerungspotenzial von Boden und Wasser (AP)", "lang": "de"}], "type": "LCIA method data set", "refObjectId": "b5c611c6-def3-11e6-bf01-fe55135034f3", "uri": "../lciamethods/b5c611c6-def3-11e6-bf01-fe55135034f3.xml"}, "other": {"anies": [{"name": "referenceToUnitGroupDataSet", "value": {"shortDescription": [{"value": "mol H^(+) eq", "lang": "en"}], "type": "unit group data set", "refObjectId": "42e089ac-92bf-4bf2-8ca1-5fc40d18f2ed", "uri": "../unitgroups/42e089ac-92bf-4bf2-8ca1-5fc40d18f2ed.xml"}}, {"value": "0.0307028953785515", "module": "A1-A3"}, {"value": "0", "module": "C1"}, {"value": "1.94929041116678E-05", "module": "C2"}, {"value": "0.000271634093164047", "module": "C3"}, {"value": "2.31523962944421E-06", "module": "C4"}, {"value": "-0.00464607853689669", "module": "D"}]}}, {"referenceToLCIAMethodDataSet": {"shortDescription": [{"value": "Eutrophication potential aquatic freshwater (EP-freshwater)", "lang": "en"}, {"value": "Eutrophierungspotenzial Süßwasser (EP-freshwater)", "lang": "de"}], "type": "LCIA method data set", "refObjectId": "b53ec18f-7377-4ad3-86eb-cc3f4f276b2b", "uri": "../lciamethods/b53ec18f-7377-4ad3-86eb-cc3f4f276b2b.xml"}, "other": {"anies": [{"name": "referenceToUnitGroupDataSet", "value": {"shortDescription": [{"value": "kg P eq", "lang": "en"}], "type": "unit group data set", "refObjectId": "0429039d-a61d-4590-ba67-aa4a20a810a1", "uri": "../unitgroups/0429039d-a61d-4590-ba67-aa4a20a810a1.xml"}}, {"value": "0.00224115776143483", "module": "A1-A3"}, {"value": "0", "module": "C1"}, {"value": "3.01013438315831E-07", "module": "C2"}, {"value": "1.49239863231408E-05", "module": "C3"}, {"value": "2.55779386052499E-08", "module": "C4"}, {"value": "-0.000503153691573856", "module": "D"}]}}, {"referenceToLCIAMethodDataSet": {"shortDescription": [{"value": "Eutrophication potential aquatic marine (EP-marine)", "lang": "en"}, {"value": "Eutrophierungspotenzial Salzwasser (EP-marine)", "lang": "de"}], "type": "LCIA method data set", "refObjectId": "b5c619fa-def3-11e6-bf01-fe55135034f3", "uri": "../lciamethods/b5c619fa-def3-11e6-bf01-fe55135034f3.xml"}, "other": {"anies": [{"name": "referenceToUnitGroupDataSet", "value": {"shortDescription": [{"value": "kg N eq", "lang": "en"}], "type": "unit group data set", "refObjectId": "d05bb823-ecdf-4686-8c40-bf1d9257859f", "uri": "../unitgroups/d05bb823-ecdf-4686-8c40-bf1d9257859f.xml"}}, {"value": "0.0081193913372097", "module": "A1-A3"}, {"value": "0", "module": "C1"}, {"value": "7.7479347054922E-06", "module": "C2"}, {"value": "6.07209643929466E-05", "module": "C3"}, {"value": "8.90406578520314E-07", "module": "C4"}, {"value": "-0.0010541818261792", "module": "D"}]}}, {"referenceToLCIAMethodDataSet": {"shortDescription": [{"value": "Eutrophication potential terrestrial (EP-terrestrial)", "lang": "en"}, {"value": "Eutrophierungspotenzial Land (EP-terrestrial)", "lang": "de"}], "type": "LCIA method data set", "refObjectId": "b5c614d2-def3-11e6-bf01-fe55135034f3", "uri": "../lciamethods/b5c614d2-def3-11e6-bf01-fe55135034f3.xml"}, "other": {"anies": [{"name": "referenceToUnitGroupDataSet", "value": {"shortDescription": [{"value": "mol N eq", "lang": "en"}], "type": "unit group data set", "refObjectId": "71b4d617-0ec9-4d3f-b65e-e438940c2401", "uri": "../unitgroups/71b4d617-0ec9-4d3f-b65e-e438940c2401.xml"}}, {"value": "0.0766912226152622", "module": "A1-A3"}, {"value": "0", "module": "C1"}, {"value": "8.28605284606248E-05", "module": "C2"}, {"value": "0.000678520564139863", "module": "C3"}, {"value": "9.52591534696355E-06", "module": "C4"}, {"value": "-0.0113451224076835", "module": "D"}]}}, {"referenceToLCIAMethodDataSet": {"shortDescription": [{"value": "Formation potential of tropospheric ozone photochemical oxidants (POCP)", "lang": "en"}, {"value": "Bildungspotential für troposphärisches Ozon (POCP)", "lang": "de"}], "type": "LCIA method data set", "refObjectId": "b5c610fe-def3-11e6-bf01-fe55135034f3", "uri": "../lciamethods/b5c610fe-def3-11e6-bf01-fe55135034f3.xml"}, "other": {"anies": [{"name": "referenceToUnitGroupDataSet", "value": {"shortDescription": [{"value": "kg NMVOC eq", "lang": "en"}], "type": "unit group data set", "refObjectId": "d27c25f8-fbc1-44c6-b47b-4adbae4199c6", "uri": "../unitgroups/d27c25f8-fbc1-44c6-b47b-4adbae4199c6.xml"}}, {"value": "0.0288062004845509", "module": "A1-A3"}, {"value": "0", "module": "C1"}, {"value": "2.89459159398624E-05", "module": "C2"}, {"value": "0.000201020297545416", "module": "C3"}, {"value": "3.31623432771421E-06", "module": "C4"}, {"value": "-0.00596098376439526", "module": "D"}]}}, {"referenceToLCIAMethodDataSet": {"shortDescription": [{"value": "Abiotic depletion potential for non fossil resources (ADPE)", "lang": "en"}, {"value": "Potenzial für den abiotischen Abbau nicht fossiler Ressourcen (ADPE)", "lang": "de"}], "type": "LCIA method data set", "refObjectId": "b2ad6494-c78d-11e6-9d9d-cec0c932ce01", "uri": "../lciamethods/b2ad6494-c78d-11e6-9d9d-cec0c932ce01.xml"}, "other": {"anies": [{"name": "referenceToUnitGroupDataSet", "value": {"shortDescription": [{"value": "kg Sb eq", "lang": "en"}], "type": "unit group data set", "refObjectId": "54ccd2d9-a32a-4fc2-923d-f2c8c93e89d4", "uri": "../unitgroups/54ccd2d9-a32a-4fc2-923d-f2c8c93e89d4.xml"}}, {"value": "7.05505595744703E-05", "module": "A1-A3"}, {"value": "0", "module": "C1"}, {"value": "1.33049041082401E-08", "module": "C2"}, {"value": "1.58945786480524E-06", "module": "C3"}, {"value": "4.32872291953433E-10", "module": "C4"}, {"value": "-9.74667238567364E-06", "module": "D"}]}}, {"referenceToLCIAMethodDataSet": {"shortDescription": [{"value": "Abiotic depletion potential for fossil resources (ADPF)", "lang": "en"}, {"value": "Potenzial für den abiotischen Abbau fossiler Brennstoffe (ADPF)", "lang": "de"}], "type": "LCIA method data set", "refObjectId": "b2ad6110-c78d-11e6-9d9d-cec0c932ce01", "uri": "../lciamethods/b2ad6110-c78d-11e6-9d9d-cec0c932ce01.xml"}, "other": {"anies": [{"name": "referenceToUnitGroupDataSet", "value": {"shortDescription": [{"value": "MJ", "lang": "en"}], "type": "unit group data set", "refObjectId": "93a60a57-a3c8-11da-a746-0800200c9a66", "uri": "../unitgroups/93a60a57-a3c8-11da-a746-0800200c9a66.xml"}}, {"value": "65.7901889275473", "module": "A1-A3"}, {"value": "0", "module": "C1"}, {"value": "0.0607226478453946", "module": "C2"}, {"value": "0.306780357639342", "module": "C3"}, {"value": "0.00771368408373152", "module": "C4"}, {"value": "-10.3346719305631", "module": "D"}]}}, {"referenceToLCIAMethodDataSet": {"shortDescription": [{"value": "Water use (WDP)", "lang": "en"}, {"value": "Wassernutzung (WDP)", "lang": "de"}], "type": "LCIA method data set", "refObjectId": "b2ad66ce-c78d-11e6-9d9d-cec0c932ce01", "uri": "../lciamethods/b2ad66ce-c78d-11e6-9d9d-cec0c932ce01.xml"}, "other": {"anies": [{"name": "referenceToUnitGroupDataSet", "value": {"shortDescription": [{"value": "m^(3) world eq deprived", "lang": "en"}], "type": "unit group data set", "refObjectId": "6ae2df01-888e-46c8-b17d-49fa3869b476", "uri": "../unitgroups/6ae2df01-888e-46c8-b17d-49fa3869b476.xml"}}, {"value": "2.14088648693327", "module": "A1-A3"}, {"value": "0", "module": "C1"}, {"value": "0.000307565297093965", "module": "C2"}, {"value": "0.00545549519410313", "module": "C3"}, {"value": "2.3977463676688E-05", "module": "C4"}, {"value": "-0.185768122872053", "module": "D"}]}}, {"referenceToLCIAMethodDataSet": {"shortDescription": [{"value": "Incidence of disease due to PM emissions (PM)", "lang": "en"}, {"value": "Auftreten von Krankheiten aufgrund von Feinstaubemissionen (PM)", "lang": "de"}], "type": "LCIA method data set", "refObjectId": "b5c602c6-def3-11e6-bf01-fe55135034f3", "uri": "../lciamethods/b5c602c6-def3-11e6-bf01-fe55135034f3.xml"}, "other": {"anies": [{"name": "referenceToUnitGroupDataSet", "value": {"shortDescription": [{"value": "Disease incidence", "lang": "en"}], "type": "unit group data set", "refObjectId": "3883559b-648f-4afc-8ba2-0bd24f3affa3", "uri": "../unitgroups/3883559b-648f-4afc-8ba2-0bd24f3affa3.xml"}}, {"value": "4.62319701999522E-07", "module": "A1-A3"}, {"value": "0", "module": "C1"}, {"value": "4.11150967007691E-10", "module": "C2"}, {"value": "3.64970559540331E-09", "module": "C3"}, {"value": "5.06965963940398E-11", "module": "C4"}, {"value": "-7.64555804233853E-08", "module": "D"}]}}, {"referenceToLCIAMethodDataSet": {"shortDescription": [{"value": "Human exposure efficiency relative to U235 (IR)", "lang": "en"}, {"value": "Wirkung durch Exposition des Menschen mit U235 (IR)", "lang": "de"}], "type": "LCIA method data set", "refObjectId": "b5c632be-def3-11e6-bf01-fe55135034f3", "uri": "../lciamethods/b5c632be-def3-11e6-bf01-fe55135034f3.xml"}, "other": {"anies": [{"name": "referenceToUnitGroupDataSet", "value": {"shortDescription": [{"value": "kBq U235 eq", "lang": "en"}], "type": "unit group data set", "refObjectId": "456b05bf-1415-44a9-9993-02452f554c09", "uri": "../unitgroups/456b05bf-1415-44a9-9993-02452f554c09.xml"}}, {"value": "0.242235692180509", "module": "A1-A3"}, {"value": "0", "module": "C1"}, {"value": "8.34325418260501E-05", "module": "C2"}, {"value": "0.00273529970894284", "module": "C3"}, {"value": "4.85460763128544E-06", "module": "C4"}, {"value": "0.0537672818723481", "module": "D"}]}}, {"referenceToLCIAMethodDataSet": {"shortDescription": [{"value": "Comparative toxic unit for ecosystems (ETP-fw)", "lang": "en"}, {"value": "Toxizitätsvergleichseinheit für Ökosysteme (ETP-fw)", "lang": "de"}], "type": "LCIA method data set", "refObjectId": "ee1082d1-b0f7-43ca-a1f0-21e2a4a74511", "uri": "../lciamethods/ee1082d1-b0f7-43ca-a1f0-21e2a4a74511.xml"}, "other": {"anies": [{"name": "referenceToUnitGroupDataSet", "value": {"shortDescription": [{"value": "CTUe", "lang": "en"}], "type": "unit group data set", "refObjectId": "aa959ded-f1eb-4efb-9c5c-2d60be36b3e6", "uri": "../unitgroups/aa959ded-f1eb-4efb-9c5c-2d60be36b3e6.xml"}}, {"value": "41.4340482433194", "module": "A1-A3"}, {"value": "0", "module": "C1"}, {"value": "0.029455912846713", "module": "C2"}, {"value": "0.236905791458184", "module": "C3"}, {"value": "0.00357774855790072", "module": "C4"}, {"value": "-1.85188841984683", "module": "D"}]}}, {"referenceToLCIAMethodDataSet": {"shortDescription": [{"value": "Comparative toxic unit for humans (carcinogenic) (HTP-c)", "lang": "en"}, {"value": "Toxizitätsvergleichseinheit für Menschen (krebserregend) (HTP-c)", "lang": "de"}], "type": "LCIA method data set", "refObjectId": "2299222a-bbd8-474f-9d4f-4dd1f18aea7c", "uri": "../lciamethods/2299222a-bbd8-474f-9d4f-4dd1f18aea7c.xml"}, "other": {"anies": [{"name": "referenceToUnitGroupDataSet", "value": {"shortDescription": [{"value": "CTUh", "lang": "en"}], "type": "unit group data set", "refObjectId": "d4c9523e-2d7e-49fd-8469-998f547d3a70", "uri": "../unitgroups/d4c9523e-2d7e-49fd-8469-998f547d3a70.xml"}}, {"value": "3.08429524852035E-08", "module": "A1-A3"}, {"value": "0", "module": "C1"}, {"value": "2.33269956154536E-12", "module": "C2"}, {"value": "4.18571230937587E-11", "module": "C3"}, {"value": "1.38155900352751E-13", "module": "C4"}, {"value": "9.95353255897846E-09", "module": "D"}]}}, {"referenceToLCIAMethodDataSet": {"shortDescription": [{"value": "Comparative toxic unit for humans (noncarcinogenic) (HTP-nc)", "lang": "en"}, {"value": "Toxizitätsvergleichseinheit für Menschen (nicht krebserregend) (HTP-nc)", "lang": "de"}], "type": "LCIA method data set", "refObjectId": "3af763a5-b7a1-48c9-9cee-1f223481fcef", "uri": "../lciamethods/3af763a5-b7a1-48c9-9cee-1f223481fcef.xml"}, "other": {"anies": [{"name": "referenceToUnitGroupDataSet", "value": {"shortDescription": [{"value": "CTUh", "lang": "en"}], "type": "unit group data set", "refObjectId": "d4c9523e-2d7e-49fd-8469-998f547d3a70", "uri": "../unitgroups/d4c9523e-2d7e-49fd-8469-998f547d3a70.xml"}}, {"value": "1.15853340190487E-07", "module": "A1-A3"}, {"value": "0", "module": "C1"}, {"value": "4.70555843152973E-11", "module": "C2"}, {"value": "1.75262164687982E-09", "module": "C3"}, {"value": "1.65485395378063E-12", "module": "C4"}, {"value": "-8.17888417766324E-09", "module": "D"}]}}, {"referenceToLCIAMethodDataSet": {"shortDescription": [{"value": "Soil quality index (SQP)", "lang": "en"}, {"value": "Bodenqualitätsindex (SQP)", "lang": "de"}], "type": "LCIA method data set", "refObjectId": "b2ad6890-c78d-11e6-9d9d-cec0c932ce01", "uri": "../lciamethods/b2ad6890-c78d-11e6-9d9d-cec0c932ce01.xml"}, "other": {"anies": [{"name": "referenceToUnitGroupDataSet", "value": {"shortDescription": [{"value": "SQP", "lang": "en"}], "type": "unit group data set", "refObjectId": "f130951c-e67f-4f7f-8dd4-665de3974e18", "uri": "../unitgroups/f130951c-e67f-4f7f-8dd4-665de3974e18.xml"}}, {"value": "31.8620070356468", "module": "A1-A3"}, {"value": "0", "module": "C1"}, {"value": "0.0452809071055444", "module": "C2"}, {"value": "0.586875942575114", "module": "C3"}, {"value": "0.0152048169458736", "module": "C4"}, {"value": "-3.25120269946918", "module": "D"}]}}]}, "otherAttributes": {"{http://www.indata.network/EPD/2019}epd-version": "1.2"}, "version": "1.1", "locations": "../ILCDLocations.xml"}