{"processInformation": {"dataSetInformation": {"UUID": "f68415ad-b095-48e3-ac10-c1e5eed31abd", "name": {"baseName": [{"value": "ALPHA1 L, UPS3, ALPHA SOLAR", "lang": "en"}, {"value": "ALPHA 1L Model C / UPS3 Model A / Solar Model B", "lang": "de"}], "functionalUnitFlowProperties": [{"lang": "en"}]}, "classificationInformation": {"classification": [{"class": [{"value": "Gebäudetechnik", "level": 0, "classId": "8"}, {"value": "Heizung", "level": 1, "classId": "8.1"}, {"value": "Wärmeverteilung und Abgabe", "level": 2, "classId": "8.1.02"}], "name": "OEKOBAU.DAT"}, {"class": [{"value": "03 Building services engineering", "level": 0}, {"value": "Sanitary facilitys", "level": 1}, {"value": "Pumps for liquids and liquids with solids", "level": 2}], "name": "IBUCategories"}]}, "generalComment": [{"value": "ALPHA1 L model C, UPS3 model A, ALPHA SOLAR model B are high-efficiency circulator pump designed for domestic heating systems. ALPHA SOLAR model B is designed for thermal solar systems. The EPD is for a representative product of ALPHA1 L model C, UPS3 model A, ALPHA SOLAR model B calculated based on a weighted average across the following variations/product models:\nCast iron 25:180\nCast iron 32:180\nCast iron 15:130\nCast iron 20:180\nCast iron 25:130", "lang": "en"}, {"value": "ALPHA1 L, UPS3 und ALPHA Solar sind hocheffiziente Umwälzpumpen für Heizungsanlagen. Die ALPHA Solar ist für thermische Solaranlagen konzipiert. ", "lang": "de"}]}, "quantitativeReference": {"referenceToReferenceFlow": [0]}, "time": {"referenceYear": 2024, "dataSetValidUntil": 2029, "other": {"anies": [{"name": "publicationDateOfEPD", "value": 1728604800000}]}}, "geography": {"locationOfOperationSupplyOrProduction": {"location": "RER"}}, "technology": {"technologyDescriptionAndIncludedProcesses": [{"value": "ALPHA1 L, UPS3 and ALPHA Solar are highly efficient circulation pumps for heating systems. The ALPHA Solar is designed for solar thermal systems. \nTechnical data: \nThe performance data of the product according to the harmonised norms, based on the harmonisation provisions above apply. The relevant technical specifications according to the\nPCR Part B are given in the table below. Characteristics that are the same for all three models are only given once. Others are given individually for all three models. The group discrimination reported in the table below only refers to the pump model. In particular, groups 1, 2 and 3 refer to ALPHA1 L model C and UPS3 model A; groups 4 and 5 refer to ALPHA Solar model B. \nDeclared unit: \nThe declared unit is 1 piece of product, including packaging.", "lang": "en"}, {"value": "ALPHA1 L, UPS3 und ALPHA Solar sind hocheffiziente Umwälzpumpen für Heizungsanlagen. Die ALPHA Solar ist für thermische Solaranlagen konzipiert.  \nTechnische Daten: \nEs gelten die Leistungsdaten des Produkts gemäß den harmonisierten Normen, die auf den oben genannten Harmonisierungsbestimmungen basieren. Die relevanten technischen Spezifikationen gemäß PCR Teil B sind in der nachstehenden Tabelle aufgeführt. Merkmale, die für alle drei Modelle gleich sind, werden nur einmal angegeben. Andere werden für alle drei Modelle einzeln angegeben. Die in der nachstehenden Tabelle angegebene Gruppendiskriminierung bezieht sich nur auf das Pumpenmodell. Insbesondere die Gruppen 1, 2 und 3 beziehen sich auf ALPHA1 L Modell C und UPS3 Modell A; die Gruppen 4 und 5 beziehen sich auf ALPHA Solar Modell B. \nDeklarierte Einheit: \nDie deklarierte Einheit ist 1 Stück des Produkts, einschließlich Verpackung.", "lang": "de"}], "technologicalApplicability": [{"value": "ALPHA1 L model C, UPS3 model A, ALPHA SOLAR model B are high-efficiency circulator pump designed for domestic heating systems. ALPHA Solar is designed for thermal solar systems", "lang": "en"}, {"value": "ALPHA1 L Modell C, UPS3 Modell A, ALPHA SOLAR Modell B sind hocheffiziente Umwälzpumpen für Heizungsanlagen. ALPHA Solar ist für thermische Solaranlagen konzipiert", "lang": "de"}]}}, "modellingAndValidation": {"LCIMethodAndAllocation": {"typeOfDataSet": "EPD", "referenceToLCAMethodDetails": [{"shortDescription": [{"value": "Pumps for liquids and liquids with solids.pdf", "lang": "en"}], "type": "source data set", "refObjectId": "ade9bbcb-d4ac-433d-9ef4-ff50f5dcd8f4"}], "other": {"anies": [{"name": "subType", "value": "average dataset"}]}}, "dataSourcesTreatmentAndRepresentativeness": {"referenceToDataSource": [{"shortDescription": [{"value": "ecoinvent database (all versions)", "lang": "en"}], "type": "source data set", "refObjectId": "b497a91f-e14b-4b69-8f28-f50eb1576766"}, {"shortDescription": [{"value": "ecoinvent 3.8 database", "lang": "en"}], "type": "source data set", "refObjectId": "0f4c65c0-6210-450f-b886-82bf8dd5ace9"}], "useAdviceForDataSet": [{"value": "Scope: \nThe declared product is 1 piece of ALPHA1 L model C, UPS3 model A, ALPHA SOLAR model B pump. The product is assembled in Bjerringbro, Denmark, and the life cycle assessment is based on data collected at the production site and from supplier up- and downstream of the supply chain. The declaration is for a representative product calculated based on a weighted average across the variations 25-180, 32-180, 15-130, 20-130 and 25-130. \nSystem boundary: \nThis LCA is a Cradle-to-Grave study. All major steps from the extraction of natural resources to the final disposal of the product are included in the scope of the analysis, following the modular approach of EN15804+A2:2019.\nBy decision no. 20170712-n of the SVR, the modules B3, B4 and B5 are by default declared as \"MNR\" (module not relevant).\n\nModules A1-A3 refer to the product stage and includes raw materials extraction and processing, transportation and distribution, and the manufacturing process. The product stage is included in this study, and according to EN 15804:2019 + A2 the system boundary with nature is set to include those processes that provide the material and energy inputs into the system and the following manufacturing, transport up to the factory gate as well as the processing of any waste arising from those processes.\nWastes and losses are included in the modules where they occur according to the polluter pays principle and the modular approach of EN 15804:2019+A2.\n\nModule A4 regards the transportation to the construction place as well as the transport from the production site to the regional distribution centre, and finally to the point of sale.\n\nModule A5 refers to the construction and installation process of the pumps, including the transportation of packaging waste to the treatment site and the waste treatment of packaging.\nThe use of energy during application (i.e. an electric hand drill) is negligible for the selected functional unit and is therefore not included in the scope of this study. The auxiliary materials are considered capital goods. There are no direct emission considered during the application process.\n\nModules B1-B7 refer to the use stage. In this study, all use stage modules are assessed, though B1, B2 and B7 are assessed to be zero. By decision no. 20170712-n of the SVR, the modules B3, B4 and B5 are by default declared as \"MNR\" (module not relevant). The modules include the provision and transport of all materials, products and related energy and water use, as well as waste processing up to the end-of-waste state or disposal of final residues during the use stage. They also include all impacts and aspects related to the losses during the use stage (i.e. production, transport, and waste processing and disposal of the lost products and materials).\n\nModules B6 contributions to operational energy use during the use stage comes from the electricity consumption of the product. The annual electricity consumption is calculated by multiplying the average power input, which is based on a defined load profile, with the annual running hours.\n\nModule C1-C4 refers to the End-of-life stage. A product reaches the end-of-life of its service life when it no longer provides any functionality. This life cycle stage includes all activities from the end-of-life of the pump, until all materials and components are processed, reused, recycled or disposed of. In accordance with EN15804+A2 and the PCR Part A C1-C4 are included.\n\nModule D refers to the burdens and benefits beyond the system boundaries. According to EN15804:A2+2019 module D includes the reuse, recovery and/or recycling potentials, expressed in net impacts and benefits. Contributions to module D comes from waste incineration processes in A5 and C4 as well as material recycling in C3. The specific fractions and net flows are shown in the scenarios section.", "lang": "en"}, {"value": "Gültigkeitsbereich: \nBei dem deklarierten Produkt handelt es sich um 1 Stück der Pumpen ALPHA1 L Modell C, UPS3 Modell A, ALPHA SOLAR Modell B. Das Produkt wird in Bjerringbro, Dänemark, zusammengebaut. Die Ökobilanz basiert auf Daten, die am Produktionsstandort und von Lieferanten vor- und nachgelagert in der Lieferkette gesammelt wurden. Die Deklaration bezieht sich auf ein repräsentatives Produkt, das auf der Grundlage eines gewichteten Durchschnitts über die Varianten 25-180, 32-180, 15-130, 20-130 und 25-130 berechnet wurde. \nSystemgrenze: \nDiese LCA ist eine Cradle-to-Grave-Studie. Alle wichtigen Schritte von der Gewinnung natürlicher Ressourcen bis zur endgültigen Entsorgung des Produkts werden in den Umfang der Analyse einbezogen, wobei der modulare Ansatz der EN15804+A2:2019 verfolgt wird. Durch den Beschluss Nr. 20170712-n des SVR werden die Module B3, B4 und B5 standardmäßig als \"MNR\" (Modul nicht relevant) deklariert. Die Module A1-A3 beziehen sich auf die Produktphase und umfassen die Rohstoffgewinnung und -verarbeitung, den Transport und Vertrieb sowie den Herstellungsprozess. Die Produktphase ist in dieser Studie enthalten, und gemäß EN 15804:2019+A2 wird die Systemgrenze mit der Natur so festgelegt, dass sie die Prozesse umfasst, die die Material- und Energiezufuhr in das System und die anschließende Herstellung, den Transport bis zum Werkstor sowie die Verarbeitung aller bei diesen Prozessen anfallenden Abfälle ermöglichen. Abfälle und Verluste werden gemäß dem Verursacherprinzip und dem modularen Ansatz der EN 15804:2019+A2 in die Module aufgenommen, in denen sie anfallen.\n\nModul A4 betrifft den Transport zur Baustelle sowie den Transport von der Produktionsstätte zum regionalen Vertriebszentrum und schließlich zum Verkaufsort. Modul A5 bezieht sich auf den Bau und die Installation der Pumpen, einschließlich des Transports der Verpackungsabfälle zur Aufbereitungsstelle und der Abfallbehandlung der Verpackungen. Der Energieverbrauch bei der Anwendung (z.B. einer elektrischen Handbohrmaschine) ist für die gewählte Funktionseinheit vernachlässigbar und wird daher nicht in den Umfang dieser Studie einbezogen. Die Hilfsstoffe werden als Investitionsgüter betrachtet. Es werden keine direkten Emissionen während des Anwendungsprozesses berücksichtigt. Die Module B1-B7 beziehen sich auf die Nutzungsphase. In dieser Studie werden alle Module der Nutzungsphase bewertet, wobei B1, B2 und B7 mit Null bewertet werden. Durch den Beschluss Nr. 20170712-n des SVR werden die Module B3, B4 und B5 standardmäßig als \"MNR\" (Modul nicht relevant) deklariert. Die Module umfassen die Bereitstellung und den Transport aller Materialien, Produkte und den damit verbundenen Energie- und Wasserverbrauch sowie die Abfallverarbeitung bis zum End-of-Waste-Zustand bzw. die Entsorgung von Endresten während der Nutzungsphase. Sie umfassen auch alle Auswirkungen und Aspekte im Zusammenhang mit den Verlusten während der Nutzungsphase (d.h. Produktion, Transport, Abfallverarbeitung und Entsorgung der verlorenen Produkte und Materialien). Die Beiträge des Moduls B6 zum betrieblichen Energieverbrauch während der Nutzungsphase stammen aus dem Stromverbrauch des Produkts. Der jährliche Stromverbrauch wird berechnet, indem die durchschnittliche Leistungsaufnahme, die auf einem definierten Lastprofil basiert, mit den jährlichen Betriebsstunden multipliziert wird. Modul C1-C4 bezieht sich auf die End-of-Life-Phase. Ein Produkt erreicht das Ende seiner Lebensdauer, wenn es keine Funktionalität mehr bietet. Diese Lebenszyklusphase umfasst alle Aktivitäten ab dem Ende der Lebensdauer der Pumpe, bis alle Materialien und Komponenten verarbeitet, wiederverwendet, recycelt oder entsorgt sind. Gemäß EN15804+A2 und der PCR Teil A sind C1-C4 enthalten. Modul D bezieht sich auf die Belastungen und Vorteile über die Systemgrenzen hinaus. Gemäß EN15804:A2+2019 umfasst Modul D die Wiederverwendungs-, Verwertungs- und/oder Recyclingpotenziale, ausgedrückt in Nettoauswirkungen und Nutzen. Die Beiträge zu Modul D stammen aus den Abfallverbrennungsprozessen in A5 und C4 sowie aus dem Materialrecycling in C3. Die spezifischen Fraktionen und Nettoströme sind im Abschnitt Szenarien aufgeführt.", "lang": "de"}], "other": {"anies": [{"name": "referenceToOriginalEPD", "value": {"shortDescription": {"value": "ALPHA1 L, UPS3, ALPHA SOLAR.pdf", "defaultValue": "ALPHA1 L, UPS3, ALPHA SOLAR.pdf", "lstrings": [{"lang": "en", "value": "ALPHA1 L, UPS3, ALPHA SOLAR.pdf"}]}, "type": "source data set", "uuid": {"uuid": "33fdd3e5-c659-42f7-a138-1f831ca341f3"}, "refObjectId": "33fdd3e5-c659-42f7-a138-1f831ca341f3", "resourceURLs": ["https://oekobaudat.de/OEKOBAU.DAT/resource/sources/33fdd3e5-c659-42f7-a138-1f831ca341f3/ALPHA1_L_UPS3_ALPHA_SOLAR_22848.pdf?version=00.02.000"]}}]}}, "validation": {"review": [{"referenceToNameOfReviewerAndInstitution": [{"shortDescription": [{"value": "Institut Bauen und Umwelt e. V.", "lang": "en"}], "type": "contact data set", "refObjectId": "d111dbec-b024-4be5-86c5-752d6eb2cf95", "uri": "../contacts/d111dbec-b024-4be5-86c5-752d6eb2cf95.xml"}], "type": "Accredited third party review"}]}, "complianceDeclarations": {"compliance": [{"referenceToComplianceSystem": {"shortDescription": [{"value": "DIN EN 15804+A2", "lang": "en"}], "type": "source data set", "refObjectId": "c0016b33-8cf7-415c-ac6e-deba0d21440d", "uri": "../sources/c0016b33-8cf7-415c-ac6e-deba0d21440d.xml"}}, {"referenceToComplianceSystem": {"shortDescription": [{"value": "ISO 14025", "lang": "en"}], "type": "source data set", "refObjectId": "4f2eb655-6e44-4874-a95a-e28f5442cd4d", "uri": "../sources/4f2eb655-6e44-4874-a95a-e28f5442cd4d.xml"}}]}}, "administrativeInformation": {"commissionerAndGoal": {"referenceToCommissioner": [{"shortDescription": [{"value": "Grundfos Holding A/S", "lang": "en"}], "type": "contact data set", "refObjectId": "de0c5e18-bdc1-43d3-bfd4-abb2d5105bed", "uri": "../contacts/de0c5e18-bdc1-43d3-bfd4-abb2d5105bed.xml"}]}, "dataGenerator": {"referenceToPersonOrEntityGeneratingTheDataSet": [{"shortDescription": [{"value": "Ecomatters BV", "lang": "en"}], "type": "contact data set", "refObjectId": "1181faf1-76bc-4b08-adec-ffe410b38b89", "uri": "../contacts/1181faf1-76bc-4b08-adec-ffe410b38b89.xml"}]}, "dataEntryBy": {"timeStamp": 1728604800000, "referenceToDataSetFormat": [{"shortDescription": [{"value": "ILCD Format", "lang": "en"}], "type": "source data set", "refObjectId": "a97a0155-0234-4b87-b4ce-a45da52f2a40", "uri": "../sources/a97a0155-0234-4b87-b4ce-a45da52f2a40.xml"}, {"shortDescription": [{"value": "EPD-Datenformaterweiterungen v1.2", "lang": "de"}, {"value": "EPD Data Format Extensions v1.2", "lang": "en"}], "type": "source data set", "refObjectId": "a29449fd-aa2f-4de8-b5d7-4b06b43c6fde", "uri": "../sources/a29449fd-aa2f-4de8-b5d7-4b06b43c6fde.xml"}]}, "publicationAndOwnership": {"dataSetVersion": "00.01.000", "referenceToRegistrationAuthority": {"shortDescription": [{"value": "Institut Bauen und Umwelt e. V.", "lang": "en"}], "type": "contact data set", "refObjectId": "d111dbec-b024-4be5-86c5-752d6eb2cf95", "uri": "../contacts/d111dbec-b024-4be5-86c5-752d6eb2cf95.xml"}, "registrationNumber": "EPD-GRU-20240333-CCC2-EN", "referenceToOwnershipOfDataSet": {"shortDescription": [{"value": "Grundfos Holding A/S", "lang": "en"}], "type": "contact data set", "refObjectId": "de0c5e18-bdc1-43d3-bfd4-abb2d5105bed", "uri": "../contacts/de0c5e18-bdc1-43d3-bfd4-abb2d5105bed.xml"}, "copyright": true, "licenseType": "Free of charge for all users and uses", "accessRestrictions": [{"value": "None", "lang": "en"}], "other": {"anies": [{"name": "referenceToPublisher", "value": {"shortDescription": [{"value": "Institut Bauen und Umwelt e. V.", "lang": "en"}], "type": "contact data set", "refObjectId": "d111dbec-b024-4be5-86c5-752d6eb2cf95", "uri": "../contacts/d111dbec-b024-4be5-86c5-752d6eb2cf95.xml"}}]}}}, "exchanges": {"exchange": [{"dataSetInternalID": 0, "referenceToFlowDataSet": {"shortDescription": [{"value": "ALPHA1 L, UPS3, ALPHA SOLAR (ALPHA 1L model C / UPS3 model A / ALPHA Solar model B)", "lang": "en"}], "type": "flow data set", "refObjectId": "221c7c37-0b31-b1fd-172e-2896be819f4c", "uri": "../flows/221c7c37-0b31-b1fd-172e-2896be819f4c.xml"}, "meanAmount": 1.0, "referencesToDataSource": {}, "referenceFlow": true, "resolvedFlowVersion": "00.01.000", "resultingflowAmount": 1.0, "flowProperties": [{"name": [{"lang": "de", "value": "Anzahl"}, {"lang": "en", "value": "Number of pieces"}], "uuid": "01846770-4cfe-4a25-8ad9-919d8d378345", "referenceFlowProperty": true, "meanValue": 1.0, "referenceUnit": "pcs.", "unitGroupUUID": "934110e3-baf4-49e9-992c-3d8109a6aafb"}], "materialProperties": [{"name": "weight per piece", "value": "2.14", "unit": "kg"}], "typeOfFlow": "Product flow", "classification": {"classHierarchy": "Gebäudetechnik / Heizung / Wärmeverteilung und Abgabe", "name": "OEKOBAU.DAT"}}, {"dataSetInternalID": 1, "referenceToFlowDataSet": {"shortDescription": [{"value": "Renewable primary energy as energy carrier (PERE)", "lang": "en"}, {"value": "Erneuerbare Primärenergie als Energieträger (PERE)", "lang": "de"}], "type": "flow data set", "refObjectId": "20f32be5-0398-4288-9b6d-accddd195317", "uri": "../flows/20f32be5-0398-4288-9b6d-accddd195317.xml"}, "exchange direction": "INPUT", "other": {"anies": [{"name": "referenceToUnitGroupDataSet", "value": {"shortDescription": [{"value": "MJ", "lang": "en"}], "type": "unit group data set", "refObjectId": "93a60a57-a3c8-11da-a746-0800200c9a66", "uri": "../unitgroups/93a60a57-a3c8-11da-a746-0800200c9a66.xml"}}, {"value": "42.5878585395837", "module": "A1-A3"}, {"value": "0.312471028011757", "module": "A4"}, {"value": "0.00251456349052861", "module": "A5"}, {"value": "0", "module": "B1"}, {"value": "0", "module": "B2"}, {"module": "B3"}, {"module": "B4"}, {"module": "B5"}, {"value": "71.9223250152834", "module": "B6"}, {"value": "0", "module": "B7"}, {"value": "0", "module": "C1"}, {"value": "0.0846171287858277", "module": "C2"}, {"value": "0.239418229522203", "module": "C3"}, {"value": "0.00316565476755076", "module": "C4"}, {"value": "-2.05176669230747", "module": "D"}]}, "resolvedFlowVersion": "38.00.000", "flowProperties": [], "typeOfFlow": "Other flow", "classification": {"classHierarchy": "Quantities", "name": "GaBiCategories"}}, {"dataSetInternalID": 2, "referenceToFlowDataSet": {"shortDescription": [{"value": "Renewable primary energy resources as material utilization (PERM)", "lang": "en"}, {"value": "Erneuerbare Primärenergie zur stofflichen Nutzung (PERM)", "lang": "de"}], "type": "flow data set", "refObjectId": "fb3ec0de-548d-4508-aea5-00b73bf6f702", "uri": "../flows/fb3ec0de-548d-4508-aea5-00b73bf6f702.xml"}, "exchange direction": "INPUT", "other": {"anies": [{"name": "referenceToUnitGroupDataSet", "value": {"shortDescription": [{"value": "MJ", "lang": "en"}], "type": "unit group data set", "refObjectId": "93a60a57-a3c8-11da-a746-0800200c9a66", "uri": "../unitgroups/93a60a57-a3c8-11da-a746-0800200c9a66.xml"}}, {"value": "8.83785473107999E-07", "module": "A1-A3"}, {"value": "4.10831611389492E-12", "module": "A4"}, {"value": "9.32532178701866E-10", "module": "A5"}, {"value": "0", "module": "B1"}, {"value": "0", "module": "B2"}, {"module": "B3"}, {"module": "B4"}, {"module": "B5"}, {"value": "1.05673453225878E-08", "module": "B6"}, {"value": "0", "module": "B7"}, {"value": "0", "module": "C1"}, {"value": "1.11253166706149E-12", "module": "C2"}, {"value": "3.88024006918843E-08", "module": "C3"}, {"value": "1.77322742525285E-09", "module": "C4"}, {"value": "-1.57666409385762E-07", "module": "D"}]}, "resolvedFlowVersion": "38.00.000", "flowProperties": [], "typeOfFlow": "Other flow", "classification": {"classHierarchy": "Quantities", "name": "GaBiCategories"}}, {"dataSetInternalID": 3, "referenceToFlowDataSet": {"shortDescription": [{"value": "Total use of renewable primary energy resources (PERT)", "lang": "en"}, {"value": "Total erneuerbare Primärenergie (PERT)", "lang": "de"}], "type": "flow data set", "refObjectId": "53f97275-fa8a-4cdd-9024-65936002acd0", "uri": "../flows/53f97275-fa8a-4cdd-9024-65936002acd0.xml"}, "exchange direction": "INPUT", "other": {"anies": [{"name": "referenceToUnitGroupDataSet", "value": {"shortDescription": [{"value": "MJ", "lang": "en"}], "type": "unit group data set", "refObjectId": "93a60a57-a3c8-11da-a746-0800200c9a66", "uri": "../unitgroups/93a60a57-a3c8-11da-a746-0800200c9a66.xml"}}, {"value": "42.5878594233692", "module": "A1-A3"}, {"value": "0.312471028015865", "module": "A4"}, {"value": "0.00251456442306079", "module": "A5"}, {"value": "0", "module": "B1"}, {"value": "0", "module": "B2"}, {"module": "B3"}, {"module": "B4"}, {"module": "B5"}, {"value": "71.9223250258508", "module": "B6"}, {"value": "0", "module": "B7"}, {"value": "0", "module": "C1"}, {"value": "0.0846171287869402", "module": "C2"}, {"value": "0.239418268324604", "module": "C3"}, {"value": "0.00316565654077818", "module": "C4"}, {"value": "-2.05176684997388", "module": "D"}]}, "resolvedFlowVersion": "38.00.000", "flowProperties": [], "typeOfFlow": "Other flow", "classification": {"classHierarchy": "Quantities / Environmental quantities / EPD EN 15804 / LCI indicators", "name": "GaBiCategories"}}, {"dataSetInternalID": 4, "referenceToFlowDataSet": {"shortDescription": [{"value": "Non renewable primary energy as energy carrier (PENRE)", "lang": "en"}, {"value": "Nicht-erneuerbare Primärenergie als Energieträger (PENRE)", "lang": "de"}], "type": "flow data set", "refObjectId": "ac857178-2b45-46ec-892a-a9a4332f0372", "uri": "../flows/ac857178-2b45-46ec-892a-a9a4332f0372.xml"}, "exchange direction": "INPUT", "other": {"anies": [{"name": "referenceToUnitGroupDataSet", "value": {"shortDescription": [{"value": "MJ", "lang": "en"}], "type": "unit group data set", "refObjectId": "93a60a57-a3c8-11da-a746-0800200c9a66", "uri": "../unitgroups/93a60a57-a3c8-11da-a746-0800200c9a66.xml"}}, {"value": "176.830157540545", "module": "A1-A3"}, {"value": "4.30975102613343", "module": "A4"}, {"value": "0.0641994149307886", "module": "A5"}, {"value": "0", "module": "B1"}, {"value": "0", "module": "B2"}, {"module": "B3"}, {"module": "B4"}, {"module": "B5"}, {"value": "525.048884715518", "module": "B6"}, {"value": "0", "module": "B7"}, {"value": "0", "module": "C1"}, {"value": "1.16708022479276", "module": "C2"}, {"value": "2.34987853182498", "module": "C3"}, {"value": "0.110135441754121", "module": "C4"}, {"value": "-29.0302123471304", "module": "D"}]}, "resolvedFlowVersion": "38.00.000", "flowProperties": [], "typeOfFlow": "Other flow", "classification": {"classHierarchy": "Quantities", "name": "GaBiCategories"}}, {"dataSetInternalID": 5, "referenceToFlowDataSet": {"shortDescription": [{"value": "Non renewable primary energy as material utilization (PENRM)", "lang": "en"}, {"value": "Nicht-erneuerbare Primärenergie zur stofflichen Nutzung (PENRM)", "lang": "de"}], "type": "flow data set", "refObjectId": "1421caa0-679d-4bf4-b282-0eb850ccae27", "uri": "../flows/1421caa0-679d-4bf4-b282-0eb850ccae27.xml"}, "exchange direction": "INPUT", "other": {"anies": [{"name": "referenceToUnitGroupDataSet", "value": {"shortDescription": [{"value": "MJ", "lang": "en"}], "type": "unit group data set", "refObjectId": "93a60a57-a3c8-11da-a746-0800200c9a66", "uri": "../unitgroups/93a60a57-a3c8-11da-a746-0800200c9a66.xml"}}, {"value": "7.61607760808834E-05", "module": "A1-A3"}, {"value": "5.11640621883555E-08", "module": "A4"}, {"value": "1.64820427068698E-10", "module": "A5"}, {"value": "0", "module": "B1"}, {"value": "0", "module": "B2"}, {"module": "B3"}, {"module": "B4"}, {"module": "B5"}, {"value": "6.27886627096006E-07", "module": "B6"}, {"value": "0", "module": "B7"}, {"value": "0", "module": "C1"}, {"value": "1.3855223848898E-08", "module": "C2"}, {"value": "0", "module": "C3"}, {"value": "0", "module": "C4"}, {"value": "-2.59272620203551E-08", "module": "D"}]}, "resolvedFlowVersion": "38.00.000", "flowProperties": [], "typeOfFlow": "Other flow", "classification": {"classHierarchy": "Quantities", "name": "GaBiCategories"}}, {"dataSetInternalID": 6, "referenceToFlowDataSet": {"shortDescription": [{"value": "Total use of non renewable primary energy resources (PENRT)", "lang": "en"}, {"value": "Total nicht erneuerbare Primärenergie (PENRT)", "lang": "de"}], "type": "flow data set", "refObjectId": "06159210-646b-4c8d-8583-da9b3b95a6c1", "uri": "../flows/06159210-646b-4c8d-8583-da9b3b95a6c1.xml"}, "exchange direction": "INPUT", "other": {"anies": [{"name": "referenceToUnitGroupDataSet", "value": {"shortDescription": [{"value": "MJ", "lang": "en"}], "type": "unit group data set", "refObjectId": "93a60a57-a3c8-11da-a746-0800200c9a66", "uri": "../unitgroups/93a60a57-a3c8-11da-a746-0800200c9a66.xml"}}, {"value": "176.855571172696", "module": "A1-A3"}, {"value": "4.30992905675096", "module": "A4"}, {"value": "0.0642145899796425", "module": "A5"}, {"value": "0", "module": "B1"}, {"value": "0", "module": "B2"}, {"module": "B3"}, {"module": "B4"}, {"module": "B5"}, {"value": "525.052813607078", "module": "B6"}, {"value": "0", "module": "B7"}, {"value": "0", "module": "C1"}, {"value": "1.1671284354694", "module": "C2"}, {"value": "2.35124192602222", "module": "C3"}, {"value": "0.110159483344337", "module": "C4"}, {"value": "-29.0321962636342", "module": "D"}]}, "resolvedFlowVersion": "38.00.000", "flowProperties": [], "typeOfFlow": "Other flow", "classification": {"classHierarchy": "Quantities / Environmental quantities / EPD EN 15804 / LCI indicators", "name": "GaBiCategories"}}, {"dataSetInternalID": 7, "referenceToFlowDataSet": {"shortDescription": [{"value": "Use of secondary material (SM)", "lang": "en"}, {"value": "Einsatz von Sekundärstoffen (SM)", "lang": "de"}], "type": "flow data set", "refObjectId": "c6a1f35f-2d09-4f54-8dfb-97e502e1ce92", "uri": "../flows/c6a1f35f-2d09-4f54-8dfb-97e502e1ce92.xml"}, "exchange direction": "INPUT", "other": {"anies": [{"name": "referenceToUnitGroupDataSet", "value": {"shortDescription": [{"value": "kg", "lang": "en"}], "type": "unit group data set", "refObjectId": "ad38d542-3fe9-439d-9b95-2f5f7752acaf", "uri": "../unitgroups/ad38d542-3fe9-439d-9b95-2f5f7752acaf.xml"}}, {"value": "1.19275409361002", "module": "A1-A3"}, {"value": "0", "module": "A4"}, {"value": "0", "module": "A5"}, {"value": "0", "module": "B1"}, {"value": "0", "module": "B2"}, {"module": "B3"}, {"module": "B4"}, {"module": "B5"}, {"value": "0", "module": "B6"}, {"value": "0", "module": "B7"}, {"value": "0", "module": "C1"}, {"value": "0", "module": "C2"}, {"value": "0", "module": "C3"}, {"value": "0", "module": "C4"}, {"value": "0", "module": "D"}]}, "resolvedFlowVersion": "38.00.000", "flowProperties": [], "typeOfFlow": "Other flow", "classification": {"classHierarchy": "Quantities / Environmental quantities / EPD EN 15804 / LCI indicators", "name": "GaBiCategories"}}, {"dataSetInternalID": 8, "referenceToFlowDataSet": {"shortDescription": [{"value": "Use of renewable secondary fuels (RSF)", "lang": "en"}, {"value": "Erneuerbare Sekundärbrennstoffe (RSF)", "lang": "de"}], "type": "flow data set", "refObjectId": "64333088-a55f-4aa2-9a31-c10b07816787", "uri": "../flows/64333088-a55f-4aa2-9a31-c10b07816787.xml"}, "exchange direction": "INPUT", "other": {"anies": [{"name": "referenceToUnitGroupDataSet", "value": {"shortDescription": [{"value": "MJ", "lang": "en"}], "type": "unit group data set", "refObjectId": "93a60a57-a3c8-11da-a746-0800200c9a66", "uri": "../unitgroups/93a60a57-a3c8-11da-a746-0800200c9a66.xml"}}, {"module": "A1-A3"}, {"module": "A4"}, {"module": "A5"}, {"value": "0", "module": "B1"}, {"value": "0", "module": "B2"}, {"module": "B3"}, {"module": "B4"}, {"module": "B5"}, {"module": "B6"}, {"value": "0", "module": "B7"}, {"value": "0", "module": "C1"}, {"module": "C2"}, {"module": "C3"}, {"module": "C4"}, {"module": "D"}]}, "resolvedFlowVersion": "38.00.000", "flowProperties": [], "typeOfFlow": "Other flow", "classification": {"classHierarchy": "Quantities / Environmental quantities / EPD EN 15804 / LCI indicators", "name": "GaBiCategories"}}, {"dataSetInternalID": 9, "referenceToFlowDataSet": {"shortDescription": [{"value": "Use of non renewable secondary fuels (NRSF)", "lang": "en"}, {"value": "Nicht erneuerbare Sekundärbrennstoffe (NRSF)", "lang": "de"}], "type": "flow data set", "refObjectId": "89def144-d39a-4287-b86f-efde453ddcb2", "uri": "../flows/89def144-d39a-4287-b86f-efde453ddcb2.xml"}, "exchange direction": "INPUT", "other": {"anies": [{"name": "referenceToUnitGroupDataSet", "value": {"shortDescription": [{"value": "MJ", "lang": "en"}], "type": "unit group data set", "refObjectId": "93a60a57-a3c8-11da-a746-0800200c9a66", "uri": "../unitgroups/93a60a57-a3c8-11da-a746-0800200c9a66.xml"}}, {"value": "0", "module": "A1-A3"}, {"value": "0", "module": "A4"}, {"value": "0", "module": "A5"}, {"value": "0", "module": "B1"}, {"value": "0", "module": "B2"}, {"module": "B3"}, {"module": "B4"}, {"module": "B5"}, {"value": "0", "module": "B6"}, {"value": "0", "module": "B7"}, {"value": "0", "module": "C1"}, {"value": "0", "module": "C2"}, {"value": "0", "module": "C3"}, {"value": "0", "module": "C4"}, {"value": "0", "module": "D"}]}, "resolvedFlowVersion": "38.00.000", "flowProperties": [], "typeOfFlow": "Other flow", "classification": {"classHierarchy": "Quantities / Environmental quantities / EPD EN 15804 / LCI indicators", "name": "GaBiCategories"}}, {"dataSetInternalID": 10, "referenceToFlowDataSet": {"shortDescription": [{"value": "Use of net fresh water (FW)", "lang": "en"}, {"value": "Einsatz von Süßwasserressourcen (FW)", "lang": "de"}], "type": "flow data set", "refObjectId": "3cf952c8-f3a4-461d-8c96-96456ca62246", "uri": "../flows/3cf952c8-f3a4-461d-8c96-96456ca62246.xml"}, "exchange direction": "INPUT", "other": {"anies": [{"name": "referenceToUnitGroupDataSet", "value": {"shortDescription": [{"value": "m^3", "lang": "en"}], "type": "unit group data set", "refObjectId": "cd950537-0a98-4044-9ba7-9f9a68d0a504", "uri": "../unitgroups/cd950537-0a98-4044-9ba7-9f9a68d0a504.xml"}}, {"value": "0.185528506996864", "module": "A1-A3"}, {"value": "0.000342239991982081", "module": "A4"}, {"value": "0.000172564077094124", "module": "A5"}, {"value": "0", "module": "B1"}, {"value": "0", "module": "B2"}, {"module": "B3"}, {"module": "B4"}, {"module": "B5"}, {"value": "0.120360514353582", "module": "B6"}, {"value": "0", "module": "B7"}, {"value": "0", "module": "C1"}, {"value": "9.26785617901159E-05", "module": "C2"}, {"value": "0.00127988741198204", "module": "C3"}, {"value": "0.000621751517144152", "module": "C4"}, {"value": "-0.00383496296387631", "module": "D"}]}, "resolvedFlowVersion": "38.00.000", "flowProperties": [], "typeOfFlow": "Other flow", "classification": {"classHierarchy": "Quantities / Environmental quantities / EPD EN 15804 / LCI indicators", "name": "GaBiCategories"}}, {"dataSetInternalID": 11, "referenceToFlowDataSet": {"shortDescription": [{"value": "Hazardous waste disposed (HWD)", "lang": "en"}, {"value": "Gefährlicher Abfall zur Deponie (HWD)", "lang": "de"}], "type": "flow data set", "refObjectId": "430f9e0f-59b2-46a0-8e0d-55e0e84948fc", "uri": "../flows/430f9e0f-59b2-46a0-8e0d-55e0e84948fc.xml"}, "exchange direction": "OUTPUT", "other": {"anies": [{"name": "referenceToUnitGroupDataSet", "value": {"shortDescription": [{"value": "kg", "lang": "en"}], "type": "unit group data set", "refObjectId": "ad38d542-3fe9-439d-9b95-2f5f7752acaf", "uri": "../unitgroups/ad38d542-3fe9-439d-9b95-2f5f7752acaf.xml"}}, {"value": "3.07677509475163E-06", "module": "A1-A3"}, {"value": "1.3344908118789E-11", "module": "A4"}, {"value": "4.29894218960575E-14", "module": "A5"}, {"value": "0", "module": "B1"}, {"value": "0", "module": "B2"}, {"module": "B3"}, {"module": "B4"}, {"module": "B5"}, {"value": "3.0432988591924E-08", "module": "B6"}, {"value": "0", "module": "B7"}, {"value": "0", "module": "C1"}, {"value": "3.61380002526224E-12", "module": "C2"}, {"value": "0", "module": "C3"}, {"value": "0", "module": "C4"}, {"value": "-6.10658117297209E-10", "module": "D"}]}, "resolvedFlowVersion": "38.00.000", "flowProperties": [], "typeOfFlow": "Other flow", "classification": {"classHierarchy": "Quantities / Environmental quantities / EPD EN 15804 / LCI indicators", "name": "GaBiCategories"}}, {"dataSetInternalID": 12, "referenceToFlowDataSet": {"shortDescription": [{"value": "Non hazardous waste disposed (NHWD)", "lang": "en"}, {"value": "Entsorgter nicht gefährlicher Abfall (NHWD)", "lang": "de"}], "type": "flow data set", "refObjectId": "b29ef66b-e286-4afa-949f-62f1a7b4d7fa", "uri": "../flows/b29ef66b-e286-4afa-949f-62f1a7b4d7fa.xml"}, "exchange direction": "OUTPUT", "other": {"anies": [{"name": "referenceToUnitGroupDataSet", "value": {"shortDescription": [{"value": "kg", "lang": "en"}], "type": "unit group data set", "refObjectId": "ad38d542-3fe9-439d-9b95-2f5f7752acaf", "uri": "../unitgroups/ad38d542-3fe9-439d-9b95-2f5f7752acaf.xml"}}, {"value": "0.29110944", "module": "A1-A3"}, {"value": "0", "module": "A4"}, {"value": "0.14825", "module": "A5"}, {"value": "0", "module": "B1"}, {"value": "0", "module": "B2"}, {"module": "B3"}, {"module": "B4"}, {"module": "B5"}, {"value": "0", "module": "B6"}, {"value": "0", "module": "B7"}, {"value": "0", "module": "C1"}, {"value": "0", "module": "C2"}, {"value": "0", "module": "C3"}, {"value": "0.3610963892", "module": "C4"}, {"value": "0", "module": "D"}]}, "resolvedFlowVersion": "38.00.000", "flowProperties": [], "typeOfFlow": "Other flow", "classification": {"classHierarchy": "Quantities / Environmental quantities / EPD EN 15804 / LCI indicators", "name": "GaBiCategories"}}, {"dataSetInternalID": 13, "referenceToFlowDataSet": {"shortDescription": [{"value": "Radioactive waste disposed (RWD)", "lang": "en"}, {"value": "Entsorgter radioaktiver Abfall (RWD)", "lang": "de"}], "type": "flow data set", "refObjectId": "3449546e-52ad-4b39-b809-9fb77cea8ff6", "uri": "../flows/3449546e-52ad-4b39-b809-9fb77cea8ff6.xml"}, "exchange direction": "OUTPUT", "other": {"anies": [{"name": "referenceToUnitGroupDataSet", "value": {"shortDescription": [{"value": "kg", "lang": "en"}], "type": "unit group data set", "refObjectId": "ad38d542-3fe9-439d-9b95-2f5f7752acaf", "uri": "../unitgroups/ad38d542-3fe9-439d-9b95-2f5f7752acaf.xml"}}, {"value": "0.00320601685016634", "module": "A1-A3"}, {"value": "8.06577588250052E-06", "module": "A4"}, {"value": "2.59831719518296E-08", "module": "A5"}, {"value": "0", "module": "B1"}, {"value": "0", "module": "B2"}, {"module": "B3"}, {"module": "B4"}, {"module": "B5"}, {"value": "0.0817916439807387", "module": "B6"}, {"value": "0", "module": "B7"}, {"value": "0", "module": "C1"}, {"value": "2.18421144817781E-06", "module": "C2"}, {"value": "0", "module": "C3"}, {"value": "0", "module": "C4"}, {"value": "-0.000482560463466075", "module": "D"}]}, "resolvedFlowVersion": "38.00.000", "flowProperties": [], "typeOfFlow": "Other flow", "classification": {"classHierarchy": "Quantities / Environmental quantities / EPD EN 15804 / LCI indicators", "name": "GaBiCategories"}}, {"dataSetInternalID": 14, "referenceToFlowDataSet": {"shortDescription": [{"value": "Components for re-use (CRU)", "lang": "en"}, {"value": "Komponenten für die Wiederverwendung (CRU)", "lang": "de"}], "type": "flow data set", "refObjectId": "a2b32f97-3fc7-4af2-b209-525bc6426f33", "uri": "../flows/a2b32f97-3fc7-4af2-b209-525bc6426f33.xml"}, "exchange direction": "OUTPUT", "other": {"anies": [{"name": "referenceToUnitGroupDataSet", "value": {"shortDescription": [{"value": "kg", "lang": "en"}], "type": "unit group data set", "refObjectId": "ad38d542-3fe9-439d-9b95-2f5f7752acaf", "uri": "../unitgroups/ad38d542-3fe9-439d-9b95-2f5f7752acaf.xml"}}, {"module": "A1-A3"}, {"module": "A4"}, {"module": "A5"}, {"value": "0", "module": "B1"}, {"value": "0", "module": "B2"}, {"module": "B3"}, {"module": "B4"}, {"module": "B5"}, {"module": "B6"}, {"value": "0", "module": "B7"}, {"value": "0", "module": "C1"}, {"module": "C2"}, {"module": "C3"}, {"module": "C4"}, {"module": "D"}]}, "resolvedFlowVersion": "38.00.000", "flowProperties": [], "typeOfFlow": "Other flow", "classification": {"classHierarchy": "Quantities / Environmental quantities / EPD EN 15804 / LCI indicators", "name": "GaBiCategories"}}, {"dataSetInternalID": 15, "referenceToFlowDataSet": {"shortDescription": [{"value": "Materials for recycling (MFR)", "lang": "en"}, {"value": "Stoffe zum Recycling (MFR)", "lang": "de"}], "type": "flow data set", "refObjectId": "d7fe48a5-4103-49c8-9aae-b0b5dfdbd6ae", "uri": "../flows/d7fe48a5-4103-49c8-9aae-b0b5dfdbd6ae.xml"}, "exchange direction": "OUTPUT", "other": {"anies": [{"name": "referenceToUnitGroupDataSet", "value": {"shortDescription": [{"value": "kg", "lang": "en"}], "type": "unit group data set", "refObjectId": "ad38d542-3fe9-439d-9b95-2f5f7752acaf", "uri": "../unitgroups/ad38d542-3fe9-439d-9b95-2f5f7752acaf.xml"}}, {"value": "0", "module": "A1-A3"}, {"value": "0", "module": "A4"}, {"value": "0", "module": "A5"}, {"value": "0", "module": "B1"}, {"value": "0", "module": "B2"}, {"module": "B3"}, {"module": "B4"}, {"module": "B5"}, {"value": "0", "module": "B6"}, {"value": "0", "module": "B7"}, {"value": "0", "module": "C1"}, {"value": "0", "module": "C2"}, {"value": "1.63286707445836", "module": "C3"}, {"value": "0", "module": "C4"}, {"value": "0", "module": "D"}]}, "resolvedFlowVersion": "38.00.000", "flowProperties": [], "typeOfFlow": "Other flow", "classification": {"classHierarchy": "Quantities / Environmental quantities / EPD EN 15804 / LCI indicators", "name": "GaBiCategories"}}, {"dataSetInternalID": 16, "referenceToFlowDataSet": {"shortDescription": [{"value": "Materials for energy recovery (MER)", "lang": "en"}, {"value": "Stoffe für die Energierückgewinnung (MER)", "lang": "de"}], "type": "flow data set", "refObjectId": "59a9181c-3aaf-46ee-8b13-2b3723b6e447", "uri": "../flows/59a9181c-3aaf-46ee-8b13-2b3723b6e447.xml"}, "exchange direction": "OUTPUT", "other": {"anies": [{"name": "referenceToUnitGroupDataSet", "value": {"shortDescription": [{"value": "kg", "lang": "en"}], "type": "unit group data set", "refObjectId": "ad38d542-3fe9-439d-9b95-2f5f7752acaf", "uri": "../unitgroups/ad38d542-3fe9-439d-9b95-2f5f7752acaf.xml"}}, {"value": "0", "module": "A1-A3"}, {"value": "0", "module": "A4"}, {"value": "0", "module": "A5"}, {"value": "0", "module": "B1"}, {"value": "0", "module": "B2"}, {"module": "B3"}, {"module": "B4"}, {"module": "B5"}, {"value": "0", "module": "B6"}, {"value": "0", "module": "B7"}, {"value": "0", "module": "C1"}, {"value": "0", "module": "C2"}, {"value": "0", "module": "C3"}, {"value": "0", "module": "C4"}, {"value": "0", "module": "D"}]}, "resolvedFlowVersion": "38.00.000", "flowProperties": [], "typeOfFlow": "Other flow", "classification": {"classHierarchy": "Quantities / Environmental quantities / EPD EN 15804 / LCI indicators", "name": "GaBiCategories"}}, {"dataSetInternalID": 17, "referenceToFlowDataSet": {"shortDescription": [{"value": "Exported electrical energy (EEE)", "lang": "en"}, {"value": "Exportierte elektrische Energie (EEE)", "lang": "de"}], "type": "flow data set", "refObjectId": "4da0c987-2b76-40d6-9e9e-82a017aaaf29", "uri": "../flows/4da0c987-2b76-40d6-9e9e-82a017aaaf29.xml"}, "exchange direction": "OUTPUT", "other": {"anies": [{"name": "referenceToUnitGroupDataSet", "value": {"shortDescription": [{"value": "MJ", "lang": "en"}], "type": "unit group data set", "refObjectId": "93a60a57-a3c8-11da-a746-0800200c9a66", "uri": "../unitgroups/93a60a57-a3c8-11da-a746-0800200c9a66.xml"}}, {"value": "0", "module": "A1-A3"}, {"value": "0", "module": "A4"}, {"value": "0.2060675", "module": "A5"}, {"value": "0", "module": "B1"}, {"value": "0", "module": "B2"}, {"module": "B3"}, {"module": "B4"}, {"module": "B5"}, {"value": "0", "module": "B6"}, {"value": "0", "module": "B7"}, {"value": "0", "module": "C1"}, {"value": "0", "module": "C2"}, {"value": "0", "module": "C3"}, {"value": "0.658268113664", "module": "C4"}, {"value": "0", "module": "D"}]}, "resolvedFlowVersion": "38.00.000", "flowProperties": [], "typeOfFlow": "Other flow", "classification": {"classHierarchy": "Quantities / Environmental quantities / EPD EN 15804 / LCI indicators", "name": "GaBiCategories"}}, {"dataSetInternalID": 18, "referenceToFlowDataSet": {"shortDescription": [{"value": "Exported thermal energy (EET)", "lang": "en"}, {"value": "Exportierte thermische Energie (EET)", "lang": "de"}], "type": "flow data set", "refObjectId": "98daf38a-7a79-46d3-9a37-2b7bd0955810", "uri": "../flows/98daf38a-7a79-46d3-9a37-2b7bd0955810.xml"}, "exchange direction": "OUTPUT", "other": {"anies": [{"name": "referenceToUnitGroupDataSet", "value": {"shortDescription": [{"value": "MJ", "lang": "en"}], "type": "unit group data set", "refObjectId": "93a60a57-a3c8-11da-a746-0800200c9a66", "uri": "../unitgroups/93a60a57-a3c8-11da-a746-0800200c9a66.xml"}}, {"value": "0", "module": "A1-A3"}, {"value": "0", "module": "A4"}, {"value": "0.4225125", "module": "A5"}, {"value": "0", "module": "B1"}, {"value": "0", "module": "B2"}, {"module": "B3"}, {"module": "B4"}, {"module": "B5"}, {"value": "0", "module": "B6"}, {"value": "0", "module": "B7"}, {"value": "0", "module": "C1"}, {"value": "0", "module": "C2"}, {"value": "0", "module": "C3"}, {"value": "1.286309630272", "module": "C4"}, {"value": "0", "module": "D"}]}, "resolvedFlowVersion": "38.00.000", "flowProperties": [], "typeOfFlow": "Other flow", "classification": {"classHierarchy": "Quantities / Environmental quantities / EPD EN 15804 / LCI indicators", "name": "GaBiCategories"}}]}, "LCIAResults": {"LCIAResult": [{"referenceToLCIAMethodDataSet": {"shortDescription": [{"value": "Global Warming Potential total (GWP-total)", "lang": "en"}, {"value": "Globales Erwärmungspotenzial total (GWP-total)", "lang": "de"}], "type": "LCIA method data set", "refObjectId": "6a37f984-a4b3-458a-a20a-64418c145fa2", "uri": "../lciamethods/6a37f984-a4b3-458a-a20a-64418c145fa2.xml"}, "other": {"anies": [{"name": "referenceToUnitGroupDataSet", "value": {"shortDescription": [{"value": "kg CO_(2) eq", "lang": "en"}], "type": "unit group data set", "refObjectId": "1ebf3012-d0db-4de2-aefd-ef30cedb0be1", "uri": "../unitgroups/1ebf3012-d0db-4de2-aefd-ef30cedb0be1.xml"}}, {"value": "13.9", "module": "A1-A3"}, {"value": "0.312", "module": "A4"}, {"value": "0.189", "module": "A5"}, {"value": "0", "module": "B1"}, {"value": "0", "module": "B2"}, {"module": "B3"}, {"module": "B4"}, {"module": "B5"}, {"value": "23.6", "module": "B6"}, {"value": "0", "module": "B7"}, {"value": "0", "module": "C1"}, {"value": "0.0846", "module": "C2"}, {"value": "0.672", "module": "C3"}, {"value": "0.4", "module": "C4"}, {"value": "-1.88", "module": "D"}]}}, {"referenceToLCIAMethodDataSet": {"shortDescription": [{"value": "Global Warming Potential fossil fuels (GWP-fossil)", "lang": "en"}, {"value": "Globales Erwärmungspotenzial fossil (GWP-fossil)", "lang": "de"}], "type": "LCIA method data set", "refObjectId": "5f635281-343e-44fb-83df-1971b155e6b6", "uri": "../lciamethods/5f635281-343e-44fb-83df-1971b155e6b6.xml"}, "other": {"anies": [{"name": "referenceToUnitGroupDataSet", "value": {"shortDescription": [{"value": "kg CO_(2) eq", "lang": "en"}], "type": "unit group data set", "refObjectId": "1ebf3012-d0db-4de2-aefd-ef30cedb0be1", "uri": "../unitgroups/1ebf3012-d0db-4de2-aefd-ef30cedb0be1.xml"}}, {"value": "14", "module": "A1-A3"}, {"value": "0.314", "module": "A4"}, {"value": "0.0779", "module": "A5"}, {"value": "0", "module": "B1"}, {"value": "0", "module": "B2"}, {"module": "B3"}, {"module": "B4"}, {"module": "B5"}, {"value": "23.6", "module": "B6"}, {"value": "0", "module": "B7"}, {"value": "0", "module": "C1"}, {"value": "0.0851", "module": "C2"}, {"value": "0.673", "module": "C3"}, {"value": "0.4", "module": "C4"}, {"value": "-1.88", "module": "D"}]}}, {"referenceToLCIAMethodDataSet": {"shortDescription": [{"value": "Global Warming Potential biogenic (GWP-biogenic)", "lang": "en"}, {"value": "Globales Erwärmungspotenzial biogen (GWP-biogenic)", "lang": "de"}], "type": "LCIA method data set", "refObjectId": "2356e1ab-0185-4db5-86e5-16de51c7485c", "uri": "../lciamethods/2356e1ab-0185-4db5-86e5-16de51c7485c.xml"}, "other": {"anies": [{"name": "referenceToUnitGroupDataSet", "value": {"shortDescription": [{"value": "kg CO_(2) eq", "lang": "en"}], "type": "unit group data set", "refObjectId": "1ebf3012-d0db-4de2-aefd-ef30cedb0be1", "uri": "../unitgroups/1ebf3012-d0db-4de2-aefd-ef30cedb0be1.xml"}}, {"value": "-0.0625", "module": "A1-A3"}, {"value": "-0.00465", "module": "A4"}, {"value": "0.111", "module": "A5"}, {"value": "0", "module": "B1"}, {"value": "0", "module": "B2"}, {"module": "B3"}, {"module": "B4"}, {"module": "B5"}, {"value": "0.00918", "module": "B6"}, {"value": "0", "module": "B7"}, {"value": "0", "module": "C1"}, {"value": "-0.00126", "module": "C2"}, {"value": "-0.00117", "module": "C3"}, {"value": "3.48E-05", "module": "C4"}, {"value": "0.00182", "module": "D"}]}}, {"referenceToLCIAMethodDataSet": {"shortDescription": [{"value": "Global Warming Potential luluc (GWP-luluc)", "lang": "en"}, {"value": "Globales Erwärmungspotenzial luluc (GWP-luluc)", "lang": "de"}], "type": "LCIA method data set", "refObjectId": "4331bbdb-978a-490d-8707-eeb047f01a55", "uri": "../lciamethods/4331bbdb-978a-490d-8707-eeb047f01a55.xml"}, "other": {"anies": [{"name": "referenceToUnitGroupDataSet", "value": {"shortDescription": [{"value": "kg CO_(2) eq", "lang": "en"}], "type": "unit group data set", "refObjectId": "1ebf3012-d0db-4de2-aefd-ef30cedb0be1", "uri": "../unitgroups/1ebf3012-d0db-4de2-aefd-ef30cedb0be1.xml"}}, {"value": "0.016", "module": "A1-A3"}, {"value": "0.00292", "module": "A4"}, {"value": "1.21E-05", "module": "A5"}, {"value": "0", "module": "B1"}, {"value": "0", "module": "B2"}, {"module": "B3"}, {"module": "B4"}, {"module": "B5"}, {"value": "0.00219", "module": "B6"}, {"value": "0", "module": "B7"}, {"value": "0", "module": "C1"}, {"value": "0.00079", "module": "C2"}, {"value": "0.000301", "module": "C3"}, {"value": "4.3E-06", "module": "C4"}, {"value": "-0.000484", "module": "D"}]}}, {"referenceToLCIAMethodDataSet": {"shortDescription": [{"value": "Depletion potential of the stratospheric ozone layer (ODP)", "lang": "en"}, {"value": "Abbau Potential der stratosphärischen Ozonschicht (ODP)", "lang": "de"}], "type": "LCIA method data set", "refObjectId": "b5c629d6-def3-11e6-bf01-fe55135034f3", "uri": "../lciamethods/b5c629d6-def3-11e6-bf01-fe55135034f3.xml"}, "other": {"anies": [{"name": "referenceToUnitGroupDataSet", "value": {"shortDescription": [{"value": "kg CFC11 eq", "lang": "en"}], "type": "unit group data set", "refObjectId": "d9e957c9-7309-4474-bf3a-7777df6c4e5b", "uri": "../unitgroups/d9e957c9-7309-4474-bf3a-7777df6c4e5b.xml"}}, {"value": "2.93E-07", "module": "A1-A3"}, {"value": "4.1E-14", "module": "A4"}, {"value": "5.18E-10", "module": "A5"}, {"value": "0", "module": "B1"}, {"value": "0", "module": "B2"}, {"module": "B3"}, {"module": "B4"}, {"module": "B5"}, {"value": "2.35E-10", "module": "B6"}, {"value": "0", "module": "B7"}, {"value": "0", "module": "C1"}, {"value": "1.11E-14", "module": "C2"}, {"value": "1.11E-08", "module": "C3"}, {"value": "1.29E-09", "module": "C4"}, {"value": "-4.53E-08", "module": "D"}]}}, {"referenceToLCIAMethodDataSet": {"shortDescription": [{"value": "Acidification potential of land and water (AP)", "lang": "en"}, {"value": "Versauerungspotenzial von Boden und Wasser (AP)", "lang": "de"}], "type": "LCIA method data set", "refObjectId": "b5c611c6-def3-11e6-bf01-fe55135034f3", "uri": "../lciamethods/b5c611c6-def3-11e6-bf01-fe55135034f3.xml"}, "other": {"anies": [{"name": "referenceToUnitGroupDataSet", "value": {"shortDescription": [{"value": "mol H^(+) eq", "lang": "en"}], "type": "unit group data set", "refObjectId": "42e089ac-92bf-4bf2-8ca1-5fc40d18f2ed", "uri": "../unitgroups/42e089ac-92bf-4bf2-8ca1-5fc40d18f2ed.xml"}}, {"value": "0.121", "module": "A1-A3"}, {"value": "0.00202", "module": "A4"}, {"value": "5.33E-05", "module": "A5"}, {"value": "0", "module": "B1"}, {"value": "0", "module": "B2"}, {"module": "B3"}, {"module": "B4"}, {"module": "B5"}, {"value": "0.0364", "module": "B6"}, {"value": "0", "module": "B7"}, {"value": "0", "module": "C1"}, {"value": "0.000548", "module": "C2"}, {"value": "0.00122", "module": "C3"}, {"value": "0.000102", "module": "C4"}, {"value": "-0.00511", "module": "D"}]}}, {"referenceToLCIAMethodDataSet": {"shortDescription": [{"value": "Eutrophication potential aquatic freshwater (EP-freshwater)", "lang": "en"}, {"value": "Eutrophierungspotenzial Süßwasser (EP-freshwater)", "lang": "de"}], "type": "LCIA method data set", "refObjectId": "b53ec18f-7377-4ad3-86eb-cc3f4f276b2b", "uri": "../lciamethods/b53ec18f-7377-4ad3-86eb-cc3f4f276b2b.xml"}, "other": {"anies": [{"name": "referenceToUnitGroupDataSet", "value": {"shortDescription": [{"value": "kg P eq", "lang": "en"}], "type": "unit group data set", "refObjectId": "0429039d-a61d-4590-ba67-aa4a20a810a1", "uri": "../unitgroups/0429039d-a61d-4590-ba67-aa4a20a810a1.xml"}}, {"value": "0.00196", "module": "A1-A3"}, {"value": "1.15E-06", "module": "A4"}, {"value": "5.78E-06", "module": "A5"}, {"value": "0", "module": "B1"}, {"value": "0", "module": "B2"}, {"module": "B3"}, {"module": "B4"}, {"module": "B5"}, {"value": "2.36E-05", "module": "B6"}, {"value": "0", "module": "B7"}, {"value": "0", "module": "C1"}, {"value": "3.12E-07", "module": "C2"}, {"value": "7.79E-05", "module": "C3"}, {"value": "1.28E-06", "module": "C4"}, {"value": "-0.000384", "module": "D"}]}}, {"referenceToLCIAMethodDataSet": {"shortDescription": [{"value": "Eutrophication potential aquatic marine (EP-marine)", "lang": "en"}, {"value": "Eutrophierungspotenzial Salzwasser (EP-marine)", "lang": "de"}], "type": "LCIA method data set", "refObjectId": "b5c619fa-def3-11e6-bf01-fe55135034f3", "uri": "../lciamethods/b5c619fa-def3-11e6-bf01-fe55135034f3.xml"}, "other": {"anies": [{"name": "referenceToUnitGroupDataSet", "value": {"shortDescription": [{"value": "kg N eq", "lang": "en"}], "type": "unit group data set", "refObjectId": "d05bb823-ecdf-4686-8c40-bf1d9257859f", "uri": "../unitgroups/d05bb823-ecdf-4686-8c40-bf1d9257859f.xml"}}, {"value": "0.0296", "module": "A1-A3"}, {"value": "0.000993", "module": "A4"}, {"value": "2.74E-05", "module": "A5"}, {"value": "0", "module": "B1"}, {"value": "0", "module": "B2"}, {"module": "B3"}, {"module": "B4"}, {"module": "B5"}, {"value": "0.0103", "module": "B6"}, {"value": "0", "module": "B7"}, {"value": "0", "module": "C1"}, {"value": "0.000269", "module": "C2"}, {"value": "0.000314", "module": "C3"}, {"value": "5.53E-05", "module": "C4"}, {"value": "-0.0014", "module": "D"}]}}, {"referenceToLCIAMethodDataSet": {"shortDescription": [{"value": "Eutrophication potential terrestrial (EP-terrestrial)", "lang": "en"}, {"value": "Eutrophierungspotenzial Land (EP-terrestrial)", "lang": "de"}], "type": "LCIA method data set", "refObjectId": "b5c614d2-def3-11e6-bf01-fe55135034f3", "uri": "../lciamethods/b5c614d2-def3-11e6-bf01-fe55135034f3.xml"}, "other": {"anies": [{"name": "referenceToUnitGroupDataSet", "value": {"shortDescription": [{"value": "mol N eq", "lang": "en"}], "type": "unit group data set", "refObjectId": "71b4d617-0ec9-4d3f-b65e-e438940c2401", "uri": "../unitgroups/71b4d617-0ec9-4d3f-b65e-e438940c2401.xml"}}, {"value": "0.139", "module": "A1-A3"}, {"value": "0.011", "module": "A4"}, {"value": "0.000243", "module": "A5"}, {"value": "0", "module": "B1"}, {"value": "0", "module": "B2"}, {"module": "B3"}, {"module": "B4"}, {"module": "B5"}, {"value": "0.108", "module": "B6"}, {"value": "0", "module": "B7"}, {"value": "0", "module": "C1"}, {"value": "0.00298", "module": "C2"}, {"value": "0.00317", "module": "C3"}, {"value": "0.000479", "module": "C4"}, {"value": "-0.0147", "module": "D"}]}}, {"referenceToLCIAMethodDataSet": {"shortDescription": [{"value": "Formation potential of tropospheric ozone photochemical oxidants (POCP)", "lang": "en"}, {"value": "Bildungspotential für troposphärisches Ozon (POCP)", "lang": "de"}], "type": "LCIA method data set", "refObjectId": "b5c610fe-def3-11e6-bf01-fe55135034f3", "uri": "../lciamethods/b5c610fe-def3-11e6-bf01-fe55135034f3.xml"}, "other": {"anies": [{"name": "referenceToUnitGroupDataSet", "value": {"shortDescription": [{"value": "kg NMVOC eq", "lang": "en"}], "type": "unit group data set", "refObjectId": "d27c25f8-fbc1-44c6-b47b-4adbae4199c6", "uri": "../unitgroups/d27c25f8-fbc1-44c6-b47b-4adbae4199c6.xml"}}, {"value": "0.0447", "module": "A1-A3"}, {"value": "0.00192", "module": "A4"}, {"value": "5.81E-05", "module": "A5"}, {"value": "0", "module": "B1"}, {"value": "0", "module": "B2"}, {"module": "B3"}, {"module": "B4"}, {"module": "B5"}, {"value": "0.0284", "module": "B6"}, {"value": "0", "module": "B7"}, {"value": "0", "module": "C1"}, {"value": "0.000519", "module": "C2"}, {"value": "0.000834", "module": "C3"}, {"value": "0.000118", "module": "C4"}, {"value": "-0.00667", "module": "D"}]}}, {"referenceToLCIAMethodDataSet": {"shortDescription": [{"value": "Abiotic depletion potential for non fossil resources (ADPE)", "lang": "en"}, {"value": "Potenzial für den abiotischen Abbau nicht fossiler Ressourcen (ADPE)", "lang": "de"}], "type": "LCIA method data set", "refObjectId": "b2ad6494-c78d-11e6-9d9d-cec0c932ce01", "uri": "../lciamethods/b2ad6494-c78d-11e6-9d9d-cec0c932ce01.xml"}, "other": {"anies": [{"name": "referenceToUnitGroupDataSet", "value": {"shortDescription": [{"value": "kg Sb eq", "lang": "en"}], "type": "unit group data set", "refObjectId": "54ccd2d9-a32a-4fc2-923d-f2c8c93e89d4", "uri": "../unitgroups/54ccd2d9-a32a-4fc2-923d-f2c8c93e89d4.xml"}}, {"value": "0.00125", "module": "A1-A3"}, {"value": "2.09E-08", "module": "A4"}, {"value": "1.56E-08", "module": "A5"}, {"value": "0", "module": "B1"}, {"value": "0", "module": "B2"}, {"module": "B3"}, {"module": "B4"}, {"module": "B5"}, {"value": "1.16E-06", "module": "B6"}, {"value": "0", "module": "B7"}, {"value": "0", "module": "C1"}, {"value": "5.66E-09", "module": "C2"}, {"value": "6.34E-06", "module": "C3"}, {"value": "3.07E-08", "module": "C4"}, {"value": "-8.96E-07", "module": "D"}]}}, {"referenceToLCIAMethodDataSet": {"shortDescription": [{"value": "Abiotic depletion potential for fossil resources (ADPF)", "lang": "en"}, {"value": "Potenzial für den abiotischen Abbau fossiler Brennstoffe (ADPF)", "lang": "de"}], "type": "LCIA method data set", "refObjectId": "b2ad6110-c78d-11e6-9d9d-cec0c932ce01", "uri": "../lciamethods/b2ad6110-c78d-11e6-9d9d-cec0c932ce01.xml"}, "other": {"anies": [{"name": "referenceToUnitGroupDataSet", "value": {"shortDescription": [{"value": "MJ", "lang": "en"}], "type": "unit group data set", "refObjectId": "93a60a57-a3c8-11da-a746-0800200c9a66", "uri": "../unitgroups/93a60a57-a3c8-11da-a746-0800200c9a66.xml"}}, {"value": "177", "module": "A1-A3"}, {"value": "4.29", "module": "A4"}, {"value": "0.0641", "module": "A5"}, {"value": "0", "module": "B1"}, {"value": "0", "module": "B2"}, {"module": "B3"}, {"module": "B4"}, {"module": "B5"}, {"value": "525", "module": "B6"}, {"value": "0", "module": "B7"}, {"value": "0", "module": "C1"}, {"value": "1.16", "module": "C2"}, {"value": "2.35", "module": "C3"}, {"value": "0.11", "module": "C4"}, {"value": "-29", "module": "D"}]}}, {"referenceToLCIAMethodDataSet": {"shortDescription": [{"value": "Water use (WDP)", "lang": "en"}, {"value": "Wassernutzung (WDP)", "lang": "de"}], "type": "LCIA method data set", "refObjectId": "b2ad66ce-c78d-11e6-9d9d-cec0c932ce01", "uri": "../lciamethods/b2ad66ce-c78d-11e6-9d9d-cec0c932ce01.xml"}, "other": {"anies": [{"name": "referenceToUnitGroupDataSet", "value": {"shortDescription": [{"value": "m^(3) world eq deprived", "lang": "en"}], "type": "unit group data set", "refObjectId": "6ae2df01-888e-46c8-b17d-49fa3869b476", "uri": "../unitgroups/6ae2df01-888e-46c8-b17d-49fa3869b476.xml"}}, {"value": "7.28", "module": "A1-A3"}, {"value": "0.00381", "module": "A4"}, {"value": "0.00738", "module": "A5"}, {"value": "0", "module": "B1"}, {"value": "0", "module": "B2"}, {"module": "B3"}, {"module": "B4"}, {"module": "B5"}, {"value": "2.01", "module": "B6"}, {"value": "0", "module": "B7"}, {"value": "0", "module": "C1"}, {"value": "0.00103", "module": "C2"}, {"value": "0.055", "module": "C3"}, {"value": "0.0267", "module": "C4"}, {"value": "-0.133", "module": "D"}]}}, {"referenceToLCIAMethodDataSet": {"shortDescription": [{"value": "Incidence of disease due to PM emissions (PM)", "lang": "en"}, {"value": "Auftreten von Krankheiten aufgrund von Feinstaubemissionen (PM)", "lang": "de"}], "type": "LCIA method data set", "refObjectId": "b5c602c6-def3-11e6-bf01-fe55135034f3", "uri": "../lciamethods/b5c602c6-def3-11e6-bf01-fe55135034f3.xml"}, "other": {"anies": [{"name": "referenceToUnitGroupDataSet", "value": {"shortDescription": [{"value": "Disease incidence", "lang": "en"}], "type": "unit group data set", "refObjectId": "3883559b-648f-4afc-8ba2-0bd24f3affa3", "uri": "../unitgroups/3883559b-648f-4afc-8ba2-0bd24f3affa3.xml"}}, {"value": "1.16E-06", "module": "A1-A3"}, {"value": "7.52E-09", "module": "A4"}, {"value": "4.23E-10", "module": "A5"}, {"value": "0", "module": "B1"}, {"value": "0", "module": "B2"}, {"module": "B3"}, {"module": "B4"}, {"module": "B5"}, {"value": "3.29E-07", "module": "B6"}, {"value": "0", "module": "B7"}, {"value": "0", "module": "C1"}, {"value": "2.04E-09", "module": "C2"}, {"value": "1.2E-08", "module": "C3"}, {"value": "6.15E-10", "module": "C4"}, {"value": "-8.68E-08", "module": "D"}]}}, {"referenceToLCIAMethodDataSet": {"shortDescription": [{"value": "Human exposure efficiency relative to U235 (IR)", "lang": "en"}, {"value": "Wirkung durch Exposition des Menschen mit U235 (IR)", "lang": "de"}], "type": "LCIA method data set", "refObjectId": "b5c632be-def3-11e6-bf01-fe55135034f3", "uri": "../lciamethods/b5c632be-def3-11e6-bf01-fe55135034f3.xml"}, "other": {"anies": [{"name": "referenceToUnitGroupDataSet", "value": {"shortDescription": [{"value": "kBq U235 eq", "lang": "en"}], "type": "unit group data set", "refObjectId": "456b05bf-1415-44a9-9993-02452f554c09", "uri": "../unitgroups/456b05bf-1415-44a9-9993-02452f554c09.xml"}}, {"value": "0.891", "module": "A1-A3"}, {"value": "0.0012", "module": "A4"}, {"value": "0.000156", "module": "A5"}, {"value": "0", "module": "B1"}, {"value": "0", "module": "B2"}, {"module": "B3"}, {"module": "B4"}, {"module": "B5"}, {"value": "12.3", "module": "B6"}, {"value": "0", "module": "B7"}, {"value": "0", "module": "C1"}, {"value": "0.000326", "module": "C2"}, {"value": "0.0174", "module": "C3"}, {"value": "0.000355", "module": "C4"}, {"value": "-0.097", "module": "D"}]}}, {"referenceToLCIAMethodDataSet": {"shortDescription": [{"value": "Comparative toxic unit for ecosystems (ETP-fw)", "lang": "en"}, {"value": "Toxizitätsvergleichseinheit für Ökosysteme (ETP-fw)", "lang": "de"}], "type": "LCIA method data set", "refObjectId": "ee1082d1-b0f7-43ca-a1f0-21e2a4a74511", "uri": "../lciamethods/ee1082d1-b0f7-43ca-a1f0-21e2a4a74511.xml"}, "other": {"anies": [{"name": "referenceToUnitGroupDataSet", "value": {"shortDescription": [{"value": "CTUe", "lang": "en"}], "type": "unit group data set", "refObjectId": "aa959ded-f1eb-4efb-9c5c-2d60be36b3e6", "uri": "../unitgroups/aa959ded-f1eb-4efb-9c5c-2d60be36b3e6.xml"}}, {"value": "145", "module": "A1-A3"}, {"value": "3.08", "module": "A4"}, {"value": "0.325", "module": "A5"}, {"value": "0", "module": "B1"}, {"value": "0", "module": "B2"}, {"module": "B3"}, {"module": "B4"}, {"module": "B5"}, {"value": "45.7", "module": "B6"}, {"value": "0", "module": "B7"}, {"value": "0", "module": "C1"}, {"value": "0.833", "module": "C2"}, {"value": "6.42", "module": "C3"}, {"value": "0.798", "module": "C4"}, {"value": "-4.6", "module": "D"}]}}, {"referenceToLCIAMethodDataSet": {"shortDescription": [{"value": "Comparative toxic unit for humans (carcinogenic) (HTP-c)", "lang": "en"}, {"value": "Toxizitätsvergleichseinheit für Menschen (krebserregend) (HTP-c)", "lang": "de"}], "type": "LCIA method data set", "refObjectId": "2299222a-bbd8-474f-9d4f-4dd1f18aea7c", "uri": "../lciamethods/2299222a-bbd8-474f-9d4f-4dd1f18aea7c.xml"}, "other": {"anies": [{"name": "referenceToUnitGroupDataSet", "value": {"shortDescription": [{"value": "CTUh", "lang": "en"}], "type": "unit group data set", "refObjectId": "d4c9523e-2d7e-49fd-8469-998f547d3a70", "uri": "../unitgroups/d4c9523e-2d7e-49fd-8469-998f547d3a70.xml"}}, {"value": "9.86E-08", "module": "A1-A3"}, {"value": "6.25E-11", "module": "A4"}, {"value": "2.27E-11", "module": "A5"}, {"value": "0", "module": "B1"}, {"value": "0", "module": "B2"}, {"module": "B3"}, {"module": "B4"}, {"module": "B5"}, {"value": "2.71E-09", "module": "B6"}, {"value": "0", "module": "B7"}, {"value": "0", "module": "C1"}, {"value": "1.69E-11", "module": "C2"}, {"value": "2.12E-10", "module": "C3"}, {"value": "3.63E-11", "module": "C4"}, {"value": "-5.86E-09", "module": "D"}]}}, {"referenceToLCIAMethodDataSet": {"shortDescription": [{"value": "Comparative toxic unit for humans (noncarcinogenic) (HTP-nc)", "lang": "en"}, {"value": "Toxizitätsvergleichseinheit für Menschen (nicht krebserregend) (HTP-nc)", "lang": "de"}], "type": "LCIA method data set", "refObjectId": "3af763a5-b7a1-48c9-9cee-1f223481fcef", "uri": "../lciamethods/3af763a5-b7a1-48c9-9cee-1f223481fcef.xml"}, "other": {"anies": [{"name": "referenceToUnitGroupDataSet", "value": {"shortDescription": [{"value": "CTUh", "lang": "en"}], "type": "unit group data set", "refObjectId": "d4c9523e-2d7e-49fd-8469-998f547d3a70", "uri": "../unitgroups/d4c9523e-2d7e-49fd-8469-998f547d3a70.xml"}}, {"value": "2.48E-07", "module": "A1-A3"}, {"value": "2.78E-09", "module": "A4"}, {"value": "7.62E-10", "module": "A5"}, {"value": "0", "module": "B1"}, {"value": "0", "module": "B2"}, {"module": "B3"}, {"module": "B4"}, {"module": "B5"}, {"value": "8.72E-08", "module": "B6"}, {"value": "0", "module": "B7"}, {"value": "0", "module": "C1"}, {"value": "7.52E-10", "module": "C2"}, {"value": "1.9E-08", "module": "C3"}, {"value": "1.23E-09", "module": "C4"}, {"value": "-7.21E-09", "module": "D"}]}}, {"referenceToLCIAMethodDataSet": {"shortDescription": [{"value": "Soil quality index (SQP)", "lang": "en"}, {"value": "Bodenqualitätsindex (SQP)", "lang": "de"}], "type": "LCIA method data set", "refObjectId": "b2ad6890-c78d-11e6-9d9d-cec0c932ce01", "uri": "../lciamethods/b2ad6890-c78d-11e6-9d9d-cec0c932ce01.xml"}, "other": {"anies": [{"name": "referenceToUnitGroupDataSet", "value": {"shortDescription": [{"value": "SQP", "lang": "en"}], "type": "unit group data set", "refObjectId": "f130951c-e67f-4f7f-8dd4-665de3974e18", "uri": "../unitgroups/f130951c-e67f-4f7f-8dd4-665de3974e18.xml"}}, {"value": "82", "module": "A1-A3"}, {"value": "1.79", "module": "A4"}, {"value": "0.0388", "module": "A5"}, {"value": "0", "module": "B1"}, {"value": "0", "module": "B2"}, {"module": "B3"}, {"module": "B4"}, {"module": "B5"}, {"value": "71", "module": "B6"}, {"value": "0", "module": "B7"}, {"value": "0", "module": "C1"}, {"value": "0.486", "module": "C2"}, {"value": "1.6", "module": "C3"}, {"value": "0.0847", "module": "C4"}, {"value": "-3.68", "module": "D"}]}}]}, "otherAttributes": {"{http://www.indata.network/EPD/2019}epd-version": "1.2"}, "version": "1.1", "locations": "../ILCDLocations.xml"}