{"processInformation": {"dataSetInformation": {"UUID": "f6eabc0a-442a-4a72-854c-02a72600901b", "name": {"baseName": [{"value": "VELUX flat roof window CVU - solar-powered", "lang": "en"}], "functionalUnitFlowProperties": [{"lang": "en"}]}, "classificationInformation": {"classification": [{"class": [{"value": "Komponenten von Fenstern und Vorhangfassaden", "level": 0, "classId": "7"}, {"value": "Fenster", "level": 1, "classId": "7.8"}, {"value": "Sonstige Fenster", "level": 2, "classId": "7.8.05"}], "name": "OEKOBAU.DAT"}, {"class": [{"value": "02 Building products", "level": 0}, {"value": "Doors, windows, shutters, and related products", "level": 1}, {"value": "Windows and doors ", "level": 2}], "name": "IBUCategories"}]}, "generalComment": [{"value": "The solar-powered  Velux flat roof windows CVU consists of a motorised base unit made of a PUR/GRP curb with a wooden core, with integrated glazing unit and hinges on one side to allow for venting and a single layer flat or curved glass top unit on top.", "lang": "en"}]}, "quantitativeReference": {"referenceToReferenceFlow": [0]}, "time": {"referenceYear": 2022, "dataSetValidUntil": 2027, "other": {"anies": [{"name": "publicationDateOfEPD", "value": 1658707200000}]}}, "geography": {"locationOfOperationSupplyOrProduction": {"location": "RER"}}, "technology": {"technologyDescriptionAndIncludedProcesses": [{"value": "The solar-powered Velux flat roof windows CVU consists of a motorised base unit made of a PUR/GRP curb with a wooden core, with integrated glazing unit and hinges on one side to allow for venting and a single layer flat or curved glass top unit on top. Velux flat roof windows CVU are used in renovation and new build. The declaration covers 100% of solar-powered VELUX flat roof windows CVU. Base unit: PU raw material, gaskets and other minor components are produced outside Velux. Cutting and profiling of wood reinforcements are done at production site in Polen and Denmark. PUR/GRP curb with wooden core, insulating glass unit and motor and wall switch are assembled at production site in Denmark. The production and final assembly of the base unit takes place in the production site in Denmark. The final production processes includes preparation of the PU/wood frame by cutting and profiling of wood, moulding, cutting, sandblasting and painting. Assembly of GRP sash by pultrusion, profiling and drilling, cutting and mounting of gaskets and installation of glazing unit and window opener as well as packaging, stacking and wrapping of product on pallets. Top-unit: All raw materials and components are produced outside Velux. The glass top unit is assembled at production site in Slovakia. The final production processes include assembly of product, as well as packaging, stacking and wrapping of product on pallets. The factories are ISO 9001 certified. \nTechnical data: \nThe Declaration of Performance including relevant technical specifications and test methods/test standards can be downloaded from the website www.velux.com/ce. \n\nThe declared values in the table relate to the reference product incl. an average pane. For other covered product variants, specific values can be selected at the bottom of the above-mentioned download page \nDeclared unit: \nThe declared unit is 1 piece of a solar-powered VELUX flat roof window CVU with a base unit made of a polyurethane, heat-treated wood and plywood with an integrated glazing unit with 1.20 m x 1.20 m  = 1.44 m2.", "lang": "en"}], "technologicalApplicability": [{"value": "Velux flat roof windows CVU are used in renovation and new build.", "lang": "en"}]}}, "modellingAndValidation": {"LCIMethodAndAllocation": {"typeOfDataSet": "EPD", "referenceToLCAMethodDetails": [{"shortDescription": [{"value": "Windows and doors .pdf", "lang": "en"}], "type": "source data set", "refObjectId": "74fe68e9-1df1-4e78-b6d5-8630b6ccf403"}], "other": {"anies": [{"name": "subType", "value": "specific dataset"}]}}, "dataSourcesTreatmentAndRepresentativeness": {"referenceToDataSource": [{"shortDescription": [{"value": "ecoinvent database (all versions)", "lang": "en"}], "type": "source data set", "refObjectId": "b497a91f-e14b-4b69-8f28-f50eb1576766"}, {"shortDescription": [{"value": "ecoinvent 3.7.1 database", "lang": "en"}], "type": "source data set", "refObjectId": "3a4d6cdd-46ad-4ff3-8452-a0323e94f789"}], "useAdviceForDataSet": [{"value": "Scope: \nThe declaration covers 100% of solar-powered VELUX flat roof windows CVU by Østbirk Bygningsindustri, Denmark. \nSystem boundary: \nType of EPD: Cradle to gate with options, with modules C1 – C4, and module D (A1-A3, C1-C3, D and additional modules\n\n\nThe production of VELUX flat roof windows (modules A1-A3) includes raw material extraction, energy generation, waste treatment and all transports up to the factory gate. In accordance with COUNCIL REGULATION (EU) No 333/2011, secondary metals are modeled as part of the product system from the moment they are available as unmixed scrap.\n\nWaste or secondary fuels are not used for production.\n\n\nModule A4 is not declared due to large variances in transport distances between the production site and the construction site, where the product is installed.\n\n\nModule A5: The products are delivered to the construction site ready to be installed. Manual installation is assumed, and electricity consumption related to electric drilling machines, screw drivers, etc. is considered to be negligible. The combustible packaging material (plastics, wood, etc.) is assumed to be thermally treated in a municipal waste incineration plant with an efficiency R1 < 0.6 (according to the ecoinvent dataset used); the recovered energy is declared as exported energy. Metals and cardboard are recycled; it is assumed that these fractions reach the end-of-waste state after having been sorted and transported (as a conservative choice) to a recycler. No packaging waste is landfilled.\n\n\nModules B1 to B7 are not relevant for the product under consideration or no significant environmental impacts occur.\n\n\nModule C1 includes manual dismantling, with no significant environmental impact.\n\n\nModule C2 comprises the transport of the dismantled VELUX flat roof window to a sorting plant and then to a waste incineration plant for the thermally treated plastic fraction.\n\n\nModules C3/C4: given the complexity of the inventoried products, a mixed end-of-life scenario is modelled, allowing the different materials to follow their most likely path.\n\nAs a rule of thumb, metals are recycled and plastics are incinerated (also due to the very limited data availability of plastics recycling and its benefits); coated and uncoated flat glass is assumed to be recycled whereas laminated glass is assumed to be landfilled due to very limited recycling potential.\n\nMetals and flat glass recycled; it is assumed that these fractions reach the end-of-waste state after having been sorted and transported to a recycler; laminated glass is landfilled. The combustible material (plastics, wood, etc.) is assumed to be thermally treated in a municipal waste incineration plant.\n\n\nModule D includes the benefits and burdens associated with recycling metals beyond the system boundary, resulting from the treatment of recycled materials from the point of end-of-waste to the point of substitution (as loads) and substitution of primary resources (as benefits).\n\nIt also includes the benefits and burdens associated with energy recovery from plastic waste in a  municipal waste incineration plant, as modeled in Module C3.\n\nIn Module D, only net flows of metals leaving the product system are considered.", "lang": "en"}], "other": {"anies": [{"name": "referenceToOriginalEPD", "value": {"shortDescription": {"value": "VELUX flat roof window CVU - solar-powered.pdf", "defaultValue": "VELUX flat roof window CVU - solar-powered.pdf", "lstrings": [{"lang": "en", "value": "VELUX flat roof window CVU - solar-powered.pdf"}]}, "type": "source data set", "uuid": {"uuid": "d40d45cc-622a-43db-be15-307ba9ae115f"}, "refObjectId": "d40d45cc-622a-43db-be15-307ba9ae115f", "resourceURLs": ["https://oekobaudat.de/OEKOBAU.DAT/resource/sources/d40d45cc-622a-43db-be15-307ba9ae115f/VELUX_flat_roof_window_CVU_-_solar-powered_22168.pdf?version=00.02.000"]}}]}}, "validation": {"review": [{"referenceToNameOfReviewerAndInstitution": [{"shortDescription": [{"value": "Institut Bauen und Umwelt e. V.", "lang": "en"}], "type": "contact data set", "refObjectId": "d111dbec-b024-4be5-86c5-752d6eb2cf95", "uri": "../contacts/d111dbec-b024-4be5-86c5-752d6eb2cf95.xml"}], "type": "Accredited third party review"}]}, "complianceDeclarations": {"compliance": [{"referenceToComplianceSystem": {"shortDescription": [{"value": "DIN EN 15804+A2", "lang": "en"}], "type": "source data set", "refObjectId": "c0016b33-8cf7-415c-ac6e-deba0d21440d", "uri": "../sources/c0016b33-8cf7-415c-ac6e-deba0d21440d.xml"}}, {"referenceToComplianceSystem": {"shortDescription": [{"value": "ISO 14025", "lang": "en"}], "type": "source data set", "refObjectId": "4f2eb655-6e44-4874-a95a-e28f5442cd4d", "uri": "../sources/4f2eb655-6e44-4874-a95a-e28f5442cd4d.xml"}}]}}, "administrativeInformation": {"commissionerAndGoal": {"referenceToCommissioner": [{"shortDescription": [{"value": "VELUX Group", "lang": "en"}], "type": "contact data set", "refObjectId": "ab62e83b-7504-48ae-abdc-def53c14790d", "uri": "../contacts/ab62e83b-7504-48ae-abdc-def53c14790d.xml"}]}, "dataGenerator": {"referenceToPersonOrEntityGeneratingTheDataSet": [{"shortDescription": [{"value": "Dr. Frank Werner - Umwelt & Entwicklung", "lang": "en"}], "type": "contact data set", "refObjectId": "62792478-795c-4ae2-ac9a-1012d9515424", "uri": "../contacts/62792478-795c-4ae2-ac9a-1012d9515424.xml"}]}, "dataEntryBy": {"timeStamp": 1658743256229, "referenceToDataSetFormat": [{"shortDescription": [{"value": "ILCD Format", "lang": "en"}], "type": "source data set", "refObjectId": "a97a0155-0234-4b87-b4ce-a45da52f2a40", "uri": "../sources/a97a0155-0234-4b87-b4ce-a45da52f2a40.xml"}, {"shortDescription": [{"value": "EPD-Datenformaterweiterungen v1.2", "lang": "de"}, {"value": "EPD Data Format Extensions v1.2", "lang": "en"}], "type": "source data set", "refObjectId": "a29449fd-aa2f-4de8-b5d7-4b06b43c6fde", "uri": "../sources/a29449fd-aa2f-4de8-b5d7-4b06b43c6fde.xml"}]}, "publicationAndOwnership": {"dataSetVersion": "00.01.000", "referenceToRegistrationAuthority": {"shortDescription": [{"value": "Institut Bauen und Umwelt e. V.", "lang": "en"}], "type": "contact data set", "refObjectId": "d111dbec-b024-4be5-86c5-752d6eb2cf95", "uri": "../contacts/d111dbec-b024-4be5-86c5-752d6eb2cf95.xml"}, "registrationNumber": "EPD-VEL-20220141-IBJ1-EN", "referenceToOwnershipOfDataSet": {"shortDescription": [{"value": "VELUX Group", "lang": "en"}], "type": "contact data set", "refObjectId": "ab62e83b-7504-48ae-abdc-def53c14790d", "uri": "../contacts/ab62e83b-7504-48ae-abdc-def53c14790d.xml"}, "copyright": true, "licenseType": "Free of charge for all users and uses", "accessRestrictions": [{"value": "None", "lang": "en"}], "other": {"anies": [{"name": "referenceToPublisher", "value": {"shortDescription": [{"value": "Institut Bauen und Umwelt e. V.", "lang": "en"}], "type": "contact data set", "refObjectId": "d111dbec-b024-4be5-86c5-752d6eb2cf95", "uri": "../contacts/d111dbec-b024-4be5-86c5-752d6eb2cf95.xml"}}]}}}, "exchanges": {"exchange": [{"dataSetInternalID": 0, "referenceToFlowDataSet": {"shortDescription": [{"value": "VELUX flat roof window CVU - solar-powered, 1.20 m x 1.20 m = 1.44 m2 ()", "lang": "en"}], "type": "flow data set", "refObjectId": "7cf6b1a4-8d61-7b8c-eb5b-4312aa08118a", "uri": "../flows/7cf6b1a4-8d61-7b8c-eb5b-4312aa08118a.xml"}, "meanAmount": 1.0, "referencesToDataSource": {}, "referenceFlow": true, "resolvedFlowVersion": "00.01.000", "resultingflowAmount": 1.0, "flowProperties": [{"name": [{"lang": "en", "value": "Number of pieces"}, {"lang": "de", "value": "Anzahl"}], "uuid": "01846770-4cfe-4a25-8ad9-919d8d378345", "referenceFlowProperty": true, "meanValue": 1.0, "referenceUnit": "pcs.", "unitGroupUUID": "934110e3-baf4-49e9-992c-3d8109a6aafb"}], "materialProperties": [{"name": "mass reference", "value": "134.0", "unit": "kg/m^3", "unitDescription": "Kilogram per cubic meter "}], "typeOfFlow": "Product flow", "classification": {"classHierarchy": "Komponenten von Fenstern und Vorhangfassaden / Fenster / Sonstige Fenster", "name": "OEKOBAU.DAT"}}, {"dataSetInternalID": 1, "referenceToFlowDataSet": {"shortDescription": [{"value": "Renewable primary energy as energy carrier (PERE)", "lang": "en"}], "type": "flow data set", "refObjectId": "20f32be5-0398-4288-9b6d-accddd195317", "uri": "../flows/20f32be5-0398-4288-9b6d-accddd195317.xml"}, "exchange direction": "INPUT", "other": {"anies": [{"name": "referenceToUnitGroupDataSet", "value": {"shortDescription": [{"value": "MJ", "lang": "en"}], "type": "unit group data set", "refObjectId": "93a60a57-a3c8-11da-a746-0800200c9a66", "uri": "../unitgroups/93a60a57-a3c8-11da-a746-0800200c9a66.xml"}}, {"value": "409.873935843447", "module": "A1-A3"}, {"value": "0.110145898847904", "module": "A5"}, {"value": "0", "module": "B1"}, {"value": "81.0010128995491", "module": "B2"}, {"value": "25233.7020848968", "module": "B6"}, {"value": "0", "module": "C1"}, {"value": "0.292615608327145", "module": "C2"}, {"value": "3.12172061919594", "module": "C3"}, {"value": "182.29337081657", "module": "C4"}, {"value": "-230.402434321871", "module": "D"}]}, "resolvedFlowVersion": "38.00.000", "flowProperties": [], "typeOfFlow": "Other flow", "classification": {"classHierarchy": "Quantities", "name": "GaBiCategories"}}, {"dataSetInternalID": 2, "referenceToFlowDataSet": {"shortDescription": [{"value": "Renewable primary energy resources as material utilization (PERM)", "lang": "en"}], "type": "flow data set", "refObjectId": "fb3ec0de-548d-4508-aea5-00b73bf6f702", "uri": "../flows/fb3ec0de-548d-4508-aea5-00b73bf6f702.xml"}, "exchange direction": "INPUT", "other": {"anies": [{"name": "referenceToUnitGroupDataSet", "value": {"shortDescription": [{"value": "MJ", "lang": "en"}], "type": "unit group data set", "refObjectId": "93a60a57-a3c8-11da-a746-0800200c9a66", "uri": "../unitgroups/93a60a57-a3c8-11da-a746-0800200c9a66.xml"}}, {"value": "364.009440060867", "module": "A1-A3"}, {"value": "-183.906864", "module": "A5"}, {"value": "0", "module": "B1"}, {"value": "1.11022302462516E-16", "module": "B2"}, {"value": "0", "module": "B6"}, {"value": "0", "module": "C1"}, {"value": "0", "module": "C2"}, {"value": "-0.986436", "module": "C3"}, {"value": "-179.116140060867", "module": "C4"}, {"value": "0", "module": "D"}]}, "resolvedFlowVersion": "38.00.000", "flowProperties": [], "typeOfFlow": "Other flow", "classification": {"classHierarchy": "Quantities", "name": "GaBiCategories"}}, {"dataSetInternalID": 3, "referenceToFlowDataSet": {"shortDescription": [{"value": "Total use of renewable primary energy resources (PERT)", "lang": "en"}], "type": "flow data set", "refObjectId": "53f97275-fa8a-4cdd-9024-65936002acd0", "uri": "../flows/53f97275-fa8a-4cdd-9024-65936002acd0.xml"}, "exchange direction": "INPUT", "other": {"anies": [{"name": "referenceToUnitGroupDataSet", "value": {"shortDescription": [{"value": "MJ", "lang": "en"}], "type": "unit group data set", "refObjectId": "93a60a57-a3c8-11da-a746-0800200c9a66", "uri": "../unitgroups/93a60a57-a3c8-11da-a746-0800200c9a66.xml"}}, {"value": "773.883375904314", "module": "A1-A3"}, {"value": "-183.796718101152", "module": "A5"}, {"value": "0", "module": "B1"}, {"value": "82.887592899544", "module": "B2"}, {"value": "25233.7020848968", "module": "B6"}, {"value": "0", "module": "C1"}, {"value": "0.292615608327145", "module": "C2"}, {"value": "2.13528461919594", "module": "C3"}, {"value": "3.17723075570282", "module": "C4"}, {"value": "-230.402434321871", "module": "D"}]}, "resolvedFlowVersion": "38.00.000", "flowProperties": [], "typeOfFlow": "Other flow", "classification": {"classHierarchy": "Quantities / Environmental quantities / EPD EN 15804 / LCI indicators", "name": "GaBiCategories"}}, {"dataSetInternalID": 4, "referenceToFlowDataSet": {"shortDescription": [{"value": "Non renewable primary energy as energy carrier (PENRE)", "lang": "en"}], "type": "flow data set", "refObjectId": "ac857178-2b45-46ec-892a-a9a4332f0372", "uri": "../flows/ac857178-2b45-46ec-892a-a9a4332f0372.xml"}, "exchange direction": "INPUT", "other": {"anies": [{"name": "referenceToUnitGroupDataSet", "value": {"shortDescription": [{"value": "MJ", "lang": "en"}], "type": "unit group data set", "refObjectId": "93a60a57-a3c8-11da-a746-0800200c9a66", "uri": "../unitgroups/93a60a57-a3c8-11da-a746-0800200c9a66.xml"}}, {"value": "5863.10817550854", "module": "A1-A3"}, {"value": "69.5257585100803", "module": "A5"}, {"value": "0", "module": "B1"}, {"value": "399.639874557382", "module": "B2"}, {"value": "0", "module": "B6"}, {"value": "0", "module": "C1"}, {"value": "20.7067702998772", "module": "C2"}, {"value": "2.11289844915098E-05", "module": "C3"}, {"value": "522.709554504665", "module": "C4"}, {"value": "-1961.60497931388", "module": "D"}]}, "resolvedFlowVersion": "38.00.000", "flowProperties": [], "typeOfFlow": "Other flow", "classification": {"classHierarchy": "Quantities", "name": "GaBiCategories"}}, {"dataSetInternalID": 5, "referenceToFlowDataSet": {"shortDescription": [{"value": "Non renewable primary energy as material utilization (PENRM)", "lang": "en"}], "type": "flow data set", "refObjectId": "1421caa0-679d-4bf4-b282-0eb850ccae27", "uri": "../flows/1421caa0-679d-4bf4-b282-0eb850ccae27.xml"}, "exchange direction": "INPUT", "other": {"anies": [{"name": "referenceToUnitGroupDataSet", "value": {"shortDescription": [{"value": "MJ", "lang": "en"}], "type": "unit group data set", "refObjectId": "93a60a57-a3c8-11da-a746-0800200c9a66", "uri": "../unitgroups/93a60a57-a3c8-11da-a746-0800200c9a66.xml"}}, {"value": "545.1783944", "module": "A1-A3"}, {"value": "-62.4132", "module": "A5"}, {"value": "0", "module": "B1"}, {"value": "0", "module": "B2"}, {"value": "0", "module": "B6"}, {"value": "0", "module": "C1"}, {"value": "0", "module": "C2"}, {"value": "0", "module": "C3"}, {"value": "-482.7651944", "module": "C4"}, {"value": "0", "module": "D"}]}, "resolvedFlowVersion": "38.00.000", "flowProperties": [], "typeOfFlow": "Other flow", "classification": {"classHierarchy": "Quantities", "name": "GaBiCategories"}}, {"dataSetInternalID": 6, "referenceToFlowDataSet": {"shortDescription": [{"value": "Total use of non renewable primary energy resources (PENRT)", "lang": "en"}], "type": "flow data set", "refObjectId": "06159210-646b-4c8d-8583-da9b3b95a6c1", "uri": "../flows/06159210-646b-4c8d-8583-da9b3b95a6c1.xml"}, "exchange direction": "INPUT", "other": {"anies": [{"name": "referenceToUnitGroupDataSet", "value": {"shortDescription": [{"value": "MJ", "lang": "en"}], "type": "unit group data set", "refObjectId": "93a60a57-a3c8-11da-a746-0800200c9a66", "uri": "../unitgroups/93a60a57-a3c8-11da-a746-0800200c9a66.xml"}}, {"value": "6408.28656990854", "module": "A1-A3"}, {"value": "7.11255851008028", "module": "A5"}, {"value": "0", "module": "B1"}, {"value": "399.639874557382", "module": "B2"}, {"value": "0", "module": "B6"}, {"value": "0", "module": "C1"}, {"value": "20.7067702998772", "module": "C2"}, {"value": "2.11289844915098E-05", "module": "C3"}, {"value": "39.9443601046652", "module": "C4"}, {"value": "-1961.60497931388", "module": "D"}]}, "resolvedFlowVersion": "38.00.000", "flowProperties": [], "typeOfFlow": "Other flow", "classification": {"classHierarchy": "Quantities / Environmental quantities / EPD EN 15804 / LCI indicators", "name": "GaBiCategories"}}, {"dataSetInternalID": 7, "referenceToFlowDataSet": {"shortDescription": [{"value": "Use of secondary material (SM)", "lang": "en"}], "type": "flow data set", "refObjectId": "c6a1f35f-2d09-4f54-8dfb-97e502e1ce92", "uri": "../flows/c6a1f35f-2d09-4f54-8dfb-97e502e1ce92.xml"}, "exchange direction": "INPUT", "other": {"anies": [{"name": "referenceToUnitGroupDataSet", "value": {"shortDescription": [{"value": "kg", "lang": "en"}], "type": "unit group data set", "refObjectId": "ad38d542-3fe9-439d-9b95-2f5f7752acaf", "uri": "../unitgroups/ad38d542-3fe9-439d-9b95-2f5f7752acaf.xml"}}, {"value": "26.6665997684416", "module": "A1-A3"}, {"value": "0", "module": "A5"}, {"value": "0", "module": "B1"}, {"value": "1.40218191352376", "module": "B2"}, {"value": "0", "module": "B6"}, {"value": "0", "module": "C1"}, {"value": "0", "module": "C2"}, {"value": "0", "module": "C3"}, {"value": "0", "module": "C4"}, {"value": "-0.35321737110963", "module": "D"}]}, "resolvedFlowVersion": "38.00.000", "flowProperties": [], "typeOfFlow": "Other flow", "classification": {"classHierarchy": "Quantities / Environmental quantities / EPD EN 15804 / LCI indicators", "name": "GaBiCategories"}}, {"dataSetInternalID": 8, "referenceToFlowDataSet": {"shortDescription": [{"value": "Use of renewable secondary fuels (RSF)", "lang": "en"}], "type": "flow data set", "refObjectId": "64333088-a55f-4aa2-9a31-c10b07816787", "uri": "../flows/64333088-a55f-4aa2-9a31-c10b07816787.xml"}, "exchange direction": "INPUT", "other": {"anies": [{"name": "referenceToUnitGroupDataSet", "value": {"shortDescription": [{"value": "MJ", "lang": "en"}], "type": "unit group data set", "refObjectId": "93a60a57-a3c8-11da-a746-0800200c9a66", "uri": "../unitgroups/93a60a57-a3c8-11da-a746-0800200c9a66.xml"}}, {"value": "0", "module": "A1-A3"}, {"value": "0", "module": "A5"}, {"value": "0", "module": "B1"}, {"value": "0", "module": "B2"}, {"value": "0", "module": "B6"}, {"value": "0", "module": "C1"}, {"value": "0", "module": "C2"}, {"value": "0", "module": "C3"}, {"value": "0", "module": "C4"}, {"value": "0", "module": "D"}]}, "resolvedFlowVersion": "38.00.000", "flowProperties": [], "typeOfFlow": "Other flow", "classification": {"classHierarchy": "Quantities / Environmental quantities / EPD EN 15804 / LCI indicators", "name": "GaBiCategories"}}, {"dataSetInternalID": 9, "referenceToFlowDataSet": {"shortDescription": [{"value": "Use of non renewable secondary fuels (NRSF)", "lang": "en"}], "type": "flow data set", "refObjectId": "89def144-d39a-4287-b86f-efde453ddcb2", "uri": "../flows/89def144-d39a-4287-b86f-efde453ddcb2.xml"}, "exchange direction": "INPUT", "other": {"anies": [{"name": "referenceToUnitGroupDataSet", "value": {"shortDescription": [{"value": "MJ", "lang": "en"}], "type": "unit group data set", "refObjectId": "93a60a57-a3c8-11da-a746-0800200c9a66", "uri": "../unitgroups/93a60a57-a3c8-11da-a746-0800200c9a66.xml"}}, {"value": "0", "module": "A1-A3"}, {"value": "0", "module": "A5"}, {"value": "0", "module": "B1"}, {"value": "0", "module": "B2"}, {"value": "0", "module": "B6"}, {"value": "0", "module": "C1"}, {"value": "0", "module": "C2"}, {"value": "0", "module": "C3"}, {"value": "0", "module": "C4"}, {"value": "0", "module": "D"}]}, "resolvedFlowVersion": "38.00.000", "flowProperties": [], "typeOfFlow": "Other flow", "classification": {"classHierarchy": "Quantities / Environmental quantities / EPD EN 15804 / LCI indicators", "name": "GaBiCategories"}}, {"dataSetInternalID": 10, "referenceToFlowDataSet": {"shortDescription": [{"value": "Use of net fresh water (FW)", "lang": "en"}], "type": "flow data set", "refObjectId": "3cf952c8-f3a4-461d-8c96-96456ca62246", "uri": "../flows/3cf952c8-f3a4-461d-8c96-96456ca62246.xml"}, "exchange direction": "INPUT", "other": {"anies": [{"name": "referenceToUnitGroupDataSet", "value": {"shortDescription": [{"value": "m^3", "lang": "en"}], "type": "unit group data set", "refObjectId": "cd950537-0a98-4044-9ba7-9f9a68d0a504", "uri": "../unitgroups/cd950537-0a98-4044-9ba7-9f9a68d0a504.xml"}}, {"value": "4.90046066947633", "module": "A1-A3"}, {"value": "0.00156080399021652", "module": "A5"}, {"value": "0", "module": "B1"}, {"value": "1.06647890081442", "module": "B2"}, {"value": "0", "module": "B6"}, {"value": "0", "module": "C1"}, {"value": "0.002255616029409", "module": "C2"}, {"value": "0.00690068922500113", "module": "C3"}, {"value": "0.0701161941276022", "module": "C4"}, {"value": "-1.1165698073225", "module": "D"}]}, "resolvedFlowVersion": "38.00.000", "flowProperties": [], "typeOfFlow": "Other flow", "classification": {"classHierarchy": "Quantities / Environmental quantities / EPD EN 15804 / LCI indicators", "name": "GaBiCategories"}}, {"dataSetInternalID": 11, "referenceToFlowDataSet": {"shortDescription": [{"value": "Hazardous waste disposed (HWD)", "lang": "en"}], "type": "flow data set", "refObjectId": "430f9e0f-59b2-46a0-8e0d-55e0e84948fc", "uri": "../flows/430f9e0f-59b2-46a0-8e0d-55e0e84948fc.xml"}, "exchange direction": "OUTPUT", "other": {"anies": [{"name": "referenceToUnitGroupDataSet", "value": {"shortDescription": [{"value": "kg", "lang": "en"}], "type": "unit group data set", "refObjectId": "ad38d542-3fe9-439d-9b95-2f5f7752acaf", "uri": "../unitgroups/ad38d542-3fe9-439d-9b95-2f5f7752acaf.xml"}}, {"value": "0.0708890295247992", "module": "A1-A3"}, {"value": "1.9310294683152E-05", "module": "A5"}, {"value": "0", "module": "B1"}, {"value": "0.0230866697804736", "module": "B2"}, {"value": "0", "module": "B6"}, {"value": "0", "module": "C1"}, {"value": "5.27882986869169E-05", "module": "C2"}, {"value": "2.11289844915098E-05", "module": "C3"}, {"value": "8.06343005482131E-05", "module": "C4"}, {"value": "0.0198199497638652", "module": "D"}]}, "resolvedFlowVersion": "38.00.000", "flowProperties": [], "typeOfFlow": "Other flow", "classification": {"classHierarchy": "Quantities / Environmental quantities / EPD EN 15804 / LCI indicators", "name": "GaBiCategories"}}, {"dataSetInternalID": 12, "referenceToFlowDataSet": {"shortDescription": [{"value": "Non hazardous waste disposed (NHWD)", "lang": "en"}], "type": "flow data set", "refObjectId": "b29ef66b-e286-4afa-949f-62f1a7b4d7fa", "uri": "../flows/b29ef66b-e286-4afa-949f-62f1a7b4d7fa.xml"}, "exchange direction": "OUTPUT", "other": {"anies": [{"name": "referenceToUnitGroupDataSet", "value": {"shortDescription": [{"value": "kg", "lang": "en"}], "type": "unit group data set", "refObjectId": "ad38d542-3fe9-439d-9b95-2f5f7752acaf", "uri": "../unitgroups/ad38d542-3fe9-439d-9b95-2f5f7752acaf.xml"}}, {"value": "90.8608136341698", "module": "A1-A3"}, {"value": "0.539344711735112", "module": "A5"}, {"value": "0", "module": "B1"}, {"value": "8.89081798663024", "module": "B2"}, {"value": "0", "module": "B6"}, {"value": "0", "module": "C1"}, {"value": "1.38708261775934", "module": "C2"}, {"value": "0.708014555837291", "module": "C3"}, {"value": "58.1320462692676", "module": "C4"}, {"value": "-40.284393582664", "module": "D"}]}, "resolvedFlowVersion": "38.00.000", "flowProperties": [], "typeOfFlow": "Other flow", "classification": {"classHierarchy": "Quantities / Environmental quantities / EPD EN 15804 / LCI indicators", "name": "GaBiCategories"}}, {"dataSetInternalID": 13, "referenceToFlowDataSet": {"shortDescription": [{"value": "Radioactive waste disposed (RWD)", "lang": "en"}], "type": "flow data set", "refObjectId": "3449546e-52ad-4b39-b809-9fb77cea8ff6", "uri": "../flows/3449546e-52ad-4b39-b809-9fb77cea8ff6.xml"}, "exchange direction": "OUTPUT", "other": {"anies": [{"name": "referenceToUnitGroupDataSet", "value": {"shortDescription": [{"value": "kg", "lang": "en"}], "type": "unit group data set", "refObjectId": "ad38d542-3fe9-439d-9b95-2f5f7752acaf", "uri": "../unitgroups/ad38d542-3fe9-439d-9b95-2f5f7752acaf.xml"}}, {"value": "0.0469042218893043", "module": "A1-A3"}, {"value": "0.000100818526032973", "module": "A5"}, {"value": "0", "module": "B1"}, {"value": "0.00208489124664592", "module": "B2"}, {"value": "0", "module": "B6"}, {"value": "0", "module": "C1"}, {"value": "0.000298992581429097", "module": "C2"}, {"value": "0.000224998988987153", "module": "C3"}, {"value": "0.000326600673244936", "module": "C4"}, {"value": "-0.00667015819912303", "module": "D"}]}, "resolvedFlowVersion": "38.00.000", "flowProperties": [], "typeOfFlow": "Other flow", "classification": {"classHierarchy": "Quantities / Environmental quantities / EPD EN 15804 / LCI indicators", "name": "GaBiCategories"}}, {"dataSetInternalID": 14, "referenceToFlowDataSet": {"shortDescription": [{"value": "Components for re-use (CRU)", "lang": "en"}], "type": "flow data set", "refObjectId": "a2b32f97-3fc7-4af2-b209-525bc6426f33", "uri": "../flows/a2b32f97-3fc7-4af2-b209-525bc6426f33.xml"}, "exchange direction": "OUTPUT", "other": {"anies": [{"name": "referenceToUnitGroupDataSet", "value": {"shortDescription": [{"value": "kg", "lang": "en"}], "type": "unit group data set", "refObjectId": "ad38d542-3fe9-439d-9b95-2f5f7752acaf", "uri": "../unitgroups/ad38d542-3fe9-439d-9b95-2f5f7752acaf.xml"}}, {"value": "0", "module": "A1-A3"}, {"value": "0", "module": "A5"}, {"value": "0", "module": "B1"}, {"value": "0", "module": "B2"}, {"value": "0", "module": "B6"}, {"value": "0", "module": "C1"}, {"value": "0", "module": "C2"}, {"value": "0", "module": "C3"}, {"value": "0", "module": "C4"}, {"value": "0", "module": "D"}]}, "resolvedFlowVersion": "38.00.000", "flowProperties": [], "typeOfFlow": "Other flow", "classification": {"classHierarchy": "Quantities / Environmental quantities / EPD EN 15804 / LCI indicators", "name": "GaBiCategories"}}, {"dataSetInternalID": 15, "referenceToFlowDataSet": {"shortDescription": [{"value": "Materials for recycling (MFR)", "lang": "en"}], "type": "flow data set", "refObjectId": "d7fe48a5-4103-49c8-9aae-b0b5dfdbd6ae", "uri": "../flows/d7fe48a5-4103-49c8-9aae-b0b5dfdbd6ae.xml"}, "exchange direction": "OUTPUT", "other": {"anies": [{"name": "referenceToUnitGroupDataSet", "value": {"shortDescription": [{"value": "kg", "lang": "en"}], "type": "unit group data set", "refObjectId": "ad38d542-3fe9-439d-9b95-2f5f7752acaf", "uri": "../unitgroups/ad38d542-3fe9-439d-9b95-2f5f7752acaf.xml"}}, {"value": "5.24688943099535", "module": "A1-A3"}, {"value": "10.8692", "module": "A5"}, {"value": "0", "module": "B1"}, {"value": "3.5036363", "module": "B2"}, {"value": "0", "module": "B6"}, {"value": "0", "module": "C1"}, {"value": "0", "module": "C2"}, {"value": "45.5591", "module": "C3"}, {"value": "0", "module": "C4"}, {"value": "0", "module": "D"}]}, "resolvedFlowVersion": "38.00.000", "flowProperties": [], "typeOfFlow": "Other flow", "classification": {"classHierarchy": "Quantities / Environmental quantities / EPD EN 15804 / LCI indicators", "name": "GaBiCategories"}}, {"dataSetInternalID": 16, "referenceToFlowDataSet": {"shortDescription": [{"value": "Materials for energy recovery (MER)", "lang": "en"}], "type": "flow data set", "refObjectId": "59a9181c-3aaf-46ee-8b13-2b3723b6e447", "uri": "../flows/59a9181c-3aaf-46ee-8b13-2b3723b6e447.xml"}, "exchange direction": "OUTPUT", "other": {"anies": [{"name": "referenceToUnitGroupDataSet", "value": {"shortDescription": [{"value": "kg", "lang": "en"}], "type": "unit group data set", "refObjectId": "ad38d542-3fe9-439d-9b95-2f5f7752acaf", "uri": "../unitgroups/ad38d542-3fe9-439d-9b95-2f5f7752acaf.xml"}}, {"value": "0", "module": "A1-A3"}, {"value": "0", "module": "A5"}, {"value": "0", "module": "B1"}, {"value": "0", "module": "B2"}, {"value": "0", "module": "B6"}, {"value": "0", "module": "C1"}, {"value": "0", "module": "C2"}, {"value": "0", "module": "C3"}, {"value": "0", "module": "C4"}, {"value": "0", "module": "D"}]}, "resolvedFlowVersion": "38.00.000", "flowProperties": [], "typeOfFlow": "Other flow", "classification": {"classHierarchy": "Quantities / Environmental quantities / EPD EN 15804 / LCI indicators", "name": "GaBiCategories"}}, {"dataSetInternalID": 17, "referenceToFlowDataSet": {"shortDescription": [{"value": "Exported electrical energy (EEE)", "lang": "en"}], "type": "flow data set", "refObjectId": "4da0c987-2b76-40d6-9e9e-82a017aaaf29", "uri": "../flows/4da0c987-2b76-40d6-9e9e-82a017aaaf29.xml"}, "exchange direction": "OUTPUT", "other": {"anies": [{"name": "referenceToUnitGroupDataSet", "value": {"shortDescription": [{"value": "MJ", "lang": "en"}], "type": "unit group data set", "refObjectId": "93a60a57-a3c8-11da-a746-0800200c9a66", "uri": "../unitgroups/93a60a57-a3c8-11da-a746-0800200c9a66.xml"}}, {"value": "15.2043266218106", "module": "A1-A3"}, {"value": "8.113716", "module": "A5"}, {"value": "0", "module": "B1"}, {"value": "1.682319533856", "module": "B2"}, {"value": "0", "module": "B6"}, {"value": "0", "module": "C1"}, {"value": "0", "module": "C2"}, {"value": "0", "module": "C3"}, {"value": "86.0445734799128", "module": "C4"}, {"value": "0", "module": "D"}]}, "resolvedFlowVersion": "38.00.000", "flowProperties": [], "typeOfFlow": "Other flow", "classification": {"classHierarchy": "Quantities / Environmental quantities / EPD EN 15804 / LCI indicators", "name": "GaBiCategories"}}, {"dataSetInternalID": 18, "referenceToFlowDataSet": {"shortDescription": [{"value": "Exported thermal energy (EET)", "lang": "en"}], "type": "flow data set", "refObjectId": "98daf38a-7a79-46d3-9a37-2b7bd0955810", "uri": "../flows/98daf38a-7a79-46d3-9a37-2b7bd0955810.xml"}, "exchange direction": "OUTPUT", "other": {"anies": [{"name": "referenceToUnitGroupDataSet", "value": {"shortDescription": [{"value": "MJ", "lang": "en"}], "type": "unit group data set", "refObjectId": "93a60a57-a3c8-11da-a746-0800200c9a66", "uri": "../unitgroups/93a60a57-a3c8-11da-a746-0800200c9a66.xml"}}, {"value": "29.5986068876345", "module": "A1-A3"}, {"value": "15.95905524", "module": "A5"}, {"value": "0", "module": "B1"}, {"value": "3.30899311389984", "module": "B2"}, {"value": "0", "module": "B6"}, {"value": "0", "module": "C1"}, {"value": "0", "module": "C2"}, {"value": "0", "module": "C3"}, {"value": "169.243057221644", "module": "C4"}, {"value": "0", "module": "D"}]}, "resolvedFlowVersion": "38.00.000", "flowProperties": [], "typeOfFlow": "Other flow", "classification": {"classHierarchy": "Quantities / Environmental quantities / EPD EN 15804 / LCI indicators", "name": "GaBiCategories"}}]}, "LCIAResults": {"LCIAResult": [{"referenceToLCIAMethodDataSet": {"shortDescription": [{"value": "Global Warming Potential total (GWP-total)", "lang": "en"}], "type": "LCIA method data set", "refObjectId": "6a37f984-a4b3-458a-a20a-64418c145fa2", "uri": "../lciamethods/6a37f984-a4b3-458a-a20a-64418c145fa2.xml"}, "other": {"anies": [{"name": "referenceToUnitGroupDataSet", "value": {"shortDescription": [{"value": "kg CO_(2)-Äq.", "lang": "en"}], "type": "unit group data set", "refObjectId": "1ebf3012-d0db-4de2-aefd-ef30cedb0be1", "uri": "../unitgroups/1ebf3012-d0db-4de2-aefd-ef30cedb0be1.xml"}}, {"value": "455.322473083707", "module": "A1-A3"}, {"value": "21.3532722523836", "module": "A5"}, {"value": "0", "module": "B1"}, {"value": "32.1292744968462", "module": "B2"}, {"value": "0", "module": "B6"}, {"value": "0", "module": "C1"}, {"value": "1.34523998045307", "module": "C2"}, {"value": "3.10515580194721", "module": "C3"}, {"value": "64.4704809422403", "module": "C4"}, {"value": "-192.758263365372", "module": "D"}]}}, {"referenceToLCIAMethodDataSet": {"shortDescription": [{"value": "Global Warming Potential fossil fuels (GWP-fossil)", "lang": "en"}], "type": "LCIA method data set", "refObjectId": "5f635281-343e-44fb-83df-1971b155e6b6", "uri": "../lciamethods/5f635281-343e-44fb-83df-1971b155e6b6.xml"}, "other": {"anies": [{"name": "referenceToUnitGroupDataSet", "value": {"shortDescription": [{"value": "kg CO_(2)-Äq.", "lang": "en"}], "type": "unit group data set", "refObjectId": "1ebf3012-d0db-4de2-aefd-ef30cedb0be1", "uri": "../unitgroups/1ebf3012-d0db-4de2-aefd-ef30cedb0be1.xml"}}, {"value": "487.488270856717", "module": "A1-A3"}, {"value": "5.33465457391554", "module": "A5"}, {"value": "0", "module": "B1"}, {"value": "32.0865750961366", "module": "B2"}, {"value": "0", "module": "B6"}, {"value": "0", "module": "C1"}, {"value": "1.3446928192666", "module": "C2"}, {"value": "3.02661341276586", "module": "C3"}, {"value": "47.7189667846078", "module": "C4"}, {"value": "-192.154814959916", "module": "D"}]}}, {"referenceToLCIAMethodDataSet": {"shortDescription": [{"value": "Global Warming Potential biogenic (GWP-biogenic)", "lang": "en"}], "type": "LCIA method data set", "refObjectId": "2356e1ab-0185-4db5-86e5-16de51c7485c", "uri": "../lciamethods/2356e1ab-0185-4db5-86e5-16de51c7485c.xml"}, "other": {"anies": [{"name": "referenceToUnitGroupDataSet", "value": {"shortDescription": [{"value": "kg CO_(2)-Äq.", "lang": "en"}], "type": "unit group data set", "refObjectId": "1ebf3012-d0db-4de2-aefd-ef30cedb0be1", "uri": "../unitgroups/1ebf3012-d0db-4de2-aefd-ef30cedb0be1.xml"}}, {"value": "-32.8429700189113", "module": "A1-A3"}, {"value": "16.0184258666667", "module": "A5"}, {"value": "0", "module": "B1"}, {"value": "-1.38777878078145E-17", "module": "B2"}, {"value": "0", "module": "B6"}, {"value": "0", "module": "C1"}, {"value": "0", "module": "C2"}, {"value": "0.0765284666666667", "module": "C3"}, {"value": "16.748015685578", "module": "C4"}, {"value": "0", "module": "D"}]}}, {"referenceToLCIAMethodDataSet": {"shortDescription": [{"value": "Global Warming Potential luluc (GWP-luluc)", "lang": "en"}], "type": "LCIA method data set", "refObjectId": "4331bbdb-978a-490d-8707-eeb047f01a55", "uri": "../lciamethods/4331bbdb-978a-490d-8707-eeb047f01a55.xml"}, "other": {"anies": [{"name": "referenceToUnitGroupDataSet", "value": {"shortDescription": [{"value": "kg CO_(2)-Äq.", "lang": "en"}], "type": "unit group data set", "refObjectId": "1ebf3012-d0db-4de2-aefd-ef30cedb0be1", "uri": "../unitgroups/1ebf3012-d0db-4de2-aefd-ef30cedb0be1.xml"}}, {"value": "0.677172245901629", "module": "A1-A3"}, {"value": "0.000191811801404293", "module": "A5"}, {"value": "0", "module": "B1"}, {"value": "0.0426994007096455", "module": "B2"}, {"value": "0", "module": "B6"}, {"value": "0", "module": "C1"}, {"value": "0.000547161186470262", "module": "C2"}, {"value": "0.0020139225146831", "module": "C3"}, {"value": "0.00349847205449618", "module": "C4"}, {"value": "-0.603448405455468", "module": "D"}]}}, {"referenceToLCIAMethodDataSet": {"shortDescription": [{"value": "Depletion potential of the stratospheric ozone layer (ODP)", "lang": "en"}], "type": "LCIA method data set", "refObjectId": "b5c629d6-def3-11e6-bf01-fe55135034f3", "uri": "../lciamethods/b5c629d6-def3-11e6-bf01-fe55135034f3.xml"}, "other": {"anies": [{"name": "referenceToUnitGroupDataSet", "value": {"shortDescription": [{"value": "kg CFC11-Äq.", "lang": "en"}], "type": "unit group data set", "refObjectId": "d9e957c9-7309-4474-bf3a-7777df6c4e5b", "uri": "../unitgroups/d9e957c9-7309-4474-bf3a-7777df6c4e5b.xml"}}, {"value": "7.23355466397518E-05", "module": "A1-A3"}, {"value": "1.08344946618054E-07", "module": "A5"}, {"value": "0", "module": "B1"}, {"value": "5.59141595857094E-06", "module": "B2"}, {"value": "0", "module": "B6"}, {"value": "0", "module": "C1"}, {"value": "3.15411292035418E-07", "module": "C2"}, {"value": "1.14550616680696E-07", "module": "C3"}, {"value": "1.3096682980225E-06", "module": "C4"}, {"value": "-8.07929337696223E-06", "module": "D"}]}}, {"referenceToLCIAMethodDataSet": {"shortDescription": [{"value": "Acidification potential of land and water (AP)", "lang": "en"}], "type": "LCIA method data set", "refObjectId": "b5c611c6-def3-11e6-bf01-fe55135034f3", "uri": "../lciamethods/b5c611c6-def3-11e6-bf01-fe55135034f3.xml"}, "other": {"anies": [{"name": "referenceToUnitGroupDataSet", "value": {"shortDescription": [{"value": "mol H^(+)-Äq.", "lang": "en"}], "type": "unit group data set", "refObjectId": "42e089ac-92bf-4bf2-8ca1-5fc40d18f2ed", "uri": "../unitgroups/42e089ac-92bf-4bf2-8ca1-5fc40d18f2ed.xml"}}, {"value": "2.59393796225438", "module": "A1-A3"}, {"value": "0.00309026671054298", "module": "A5"}, {"value": "0", "module": "B1"}, {"value": "0.433258437371959", "module": "B2"}, {"value": "0", "module": "B6"}, {"value": "0", "module": "C1"}, {"value": "0.00762533621371607", "module": "C2"}, {"value": "0.0072051730414466", "module": "C3"}, {"value": "0.042688806656458", "module": "C4"}, {"value": "-1.06776309439816", "module": "D"}]}}, {"referenceToLCIAMethodDataSet": {"shortDescription": [{"value": "Eutrophication potential aquatic freshwater (EP-freshwater)", "lang": "en"}], "type": "LCIA method data set", "refObjectId": "b53ec18f-7377-4ad3-86eb-cc3f4f276b2b", "uri": "../lciamethods/b53ec18f-7377-4ad3-86eb-cc3f4f276b2b.xml"}, "other": {"anies": [{"name": "referenceToUnitGroupDataSet", "value": {"shortDescription": [{"value": "kg PO_(4)-Äq.", "lang": "en"}], "type": "unit group data set", "refObjectId": "0429039d-a61d-4590-ba67-aa4a20a810a1", "uri": "../unitgroups/0429039d-a61d-4590-ba67-aa4a20a810a1.xml"}}, {"value": "0.0149416612282973", "module": "A1-A3"}, {"value": "3.72151084993856E-06", "module": "A5"}, {"value": "0", "module": "B1"}, {"value": "0.00243140623581276", "module": "B2"}, {"value": "0", "module": "B6"}, {"value": "0", "module": "C1"}, {"value": "9.89074055834858E-06", "module": "C2"}, {"value": "0.000230218293041387", "module": "C3"}, {"value": "0.000106405915951363", "module": "C4"}, {"value": "-0.00886489388635", "module": "D"}]}}, {"referenceToLCIAMethodDataSet": {"shortDescription": [{"value": "Eutrophication potential aquatic marine (EP-marine)", "lang": "en"}], "type": "LCIA method data set", "refObjectId": "b5c619fa-def3-11e6-bf01-fe55135034f3", "uri": "../lciamethods/b5c619fa-def3-11e6-bf01-fe55135034f3.xml"}, "other": {"anies": [{"name": "referenceToUnitGroupDataSet", "value": {"shortDescription": [{"value": "kg N-Äq.", "lang": "en"}], "type": "unit group data set", "refObjectId": "d05bb823-ecdf-4686-8c40-bf1d9257859f", "uri": "../unitgroups/d05bb823-ecdf-4686-8c40-bf1d9257859f.xml"}}, {"value": "0.477097768906675", "module": "A1-A3"}, {"value": "0.00116692181744187", "module": "A5"}, {"value": "0", "module": "B1"}, {"value": "0.0385277827241242", "module": "B2"}, {"value": "0", "module": "B6"}, {"value": "0", "module": "C1"}, {"value": "0.00274049041674962", "module": "C2"}, {"value": "0.00235496044775064", "module": "C3"}, {"value": "0.0185500488869586", "module": "C4"}, {"value": "-0.161590003888806", "module": "D"}]}}, {"referenceToLCIAMethodDataSet": {"shortDescription": [{"value": "Eutrophication potential terrestrial (EP-terrestrial)", "lang": "en"}], "type": "LCIA method data set", "refObjectId": "b5c614d2-def3-11e6-bf01-fe55135034f3", "uri": "../lciamethods/b5c614d2-def3-11e6-bf01-fe55135034f3.xml"}, "other": {"anies": [{"name": "referenceToUnitGroupDataSet", "value": {"shortDescription": [{"value": "mol N-Äq.", "lang": "en"}], "type": "unit group data set", "refObjectId": "71b4d617-0ec9-4d3f-b65e-e438940c2401", "uri": "../unitgroups/71b4d617-0ec9-4d3f-b65e-e438940c2401.xml"}}, {"value": "4.85664826935337", "module": "A1-A3"}, {"value": "0.0129189568293947", "module": "A5"}, {"value": "0", "module": "B1"}, {"value": "0.412798459630234", "module": "B2"}, {"value": "0", "module": "B6"}, {"value": "0", "module": "C1"}, {"value": "0.0301674472870377", "module": "C2"}, {"value": "0.0265184513636694", "module": "C3"}, {"value": "0.192412463353218", "module": "C4"}, {"value": "-1.79105285691567", "module": "D"}]}}, {"referenceToLCIAMethodDataSet": {"shortDescription": [{"value": "Formation potential of tropospheric ozone photochemical oxidants (POCP)", "lang": "en"}], "type": "LCIA method data set", "refObjectId": "b5c610fe-def3-11e6-bf01-fe55135034f3", "uri": "../lciamethods/b5c610fe-def3-11e6-bf01-fe55135034f3.xml"}, "other": {"anies": [{"name": "referenceToUnitGroupDataSet", "value": {"shortDescription": [{"value": "kg NMVOC-Äq.", "lang": "en"}], "type": "unit group data set", "refObjectId": "d27c25f8-fbc1-44c6-b47b-4adbae4199c6", "uri": "../unitgroups/d27c25f8-fbc1-44c6-b47b-4adbae4199c6.xml"}}, {"value": "1.47296997213519", "module": "A1-A3"}, {"value": "0.00363124147118403", "module": "A5"}, {"value": "0", "module": "B1"}, {"value": "0.152003579642496", "module": "B2"}, {"value": "0", "module": "B6"}, {"value": "0", "module": "C1"}, {"value": "0.0086240602689628", "module": "C2"}, {"value": "0.00703851209222743", "module": "C3"}, {"value": "0.0470045065729956", "module": "C4"}, {"value": "-0.532639272771825", "module": "D"}]}}, {"referenceToLCIAMethodDataSet": {"shortDescription": [{"value": "Abiotic depletion potential for non fossil resources (ADPE)", "lang": "en"}], "type": "LCIA method data set", "refObjectId": "b2ad6494-c78d-11e6-9d9d-cec0c932ce01", "uri": "../lciamethods/b2ad6494-c78d-11e6-9d9d-cec0c932ce01.xml"}, "other": {"anies": [{"name": "referenceToUnitGroupDataSet", "value": {"shortDescription": [{"value": "kg Sb-Äq.", "lang": "en"}], "type": "unit group data set", "refObjectId": "54ccd2d9-a32a-4fc2-923d-f2c8c93e89d4", "uri": "../unitgroups/54ccd2d9-a32a-4fc2-923d-f2c8c93e89d4.xml"}}, {"value": "897.706574184779", "module": "A1-A3"}, {"value": "1.59615990601168E-06", "module": "A5"}, {"value": "0", "module": "B1"}, {"value": "0.00547750933532211", "module": "B2"}, {"value": "0", "module": "B6"}, {"value": "0", "module": "C1"}, {"value": "4.50447894574032E-06", "module": "C2"}, {"value": "3.21316098696209E-06", "module": "C3"}, {"value": "2.84988607869546E-05", "module": "C4"}, {"value": "0.00121631655318508", "module": "D"}]}}, {"referenceToLCIAMethodDataSet": {"shortDescription": [{"value": "Abiotic depletion potential for fossil resources (ADPF)", "lang": "en"}], "type": "LCIA method data set", "refObjectId": "b2ad6110-c78d-11e6-9d9d-cec0c932ce01", "uri": "../lciamethods/b2ad6110-c78d-11e6-9d9d-cec0c932ce01.xml"}, "other": {"anies": [{"name": "referenceToUnitGroupDataSet", "value": {"shortDescription": [{"value": "MJ", "lang": "en"}], "type": "unit group data set", "refObjectId": "93a60a57-a3c8-11da-a746-0800200c9a66", "uri": "../unitgroups/93a60a57-a3c8-11da-a746-0800200c9a66.xml"}}, {"value": "4767.7120852373", "module": "A1-A3"}, {"value": "7.10980780286018", "module": "A5"}, {"value": "0", "module": "B1"}, {"value": "400.6830901211", "module": "B2"}, {"value": "0", "module": "B6"}, {"value": "0", "module": "C1"}, {"value": "20.6991334185422", "module": "C2"}, {"value": "24.9737405331379", "module": "C3"}, {"value": "39.8636931618007", "module": "C4"}, {"value": "-1951.08698397034", "module": "D"}]}}, {"referenceToLCIAMethodDataSet": {"shortDescription": [{"value": "Water use (WDP)", "lang": "en"}], "type": "LCIA method data set", "refObjectId": "b2ad66ce-c78d-11e6-9d9d-cec0c932ce01", "uri": "../lciamethods/b2ad66ce-c78d-11e6-9d9d-cec0c932ce01.xml"}, "other": {"anies": [{"name": "referenceToUnitGroupDataSet", "value": {"shortDescription": [{"value": "m^(3) world-Äq. deprived", "lang": "en"}], "type": "unit group data set", "refObjectId": "6ae2df01-888e-46c8-b17d-49fa3869b476", "uri": "../unitgroups/6ae2df01-888e-46c8-b17d-49fa3869b476.xml"}}, {"value": "164.933199366925", "module": "A1-A3"}, {"value": "0.0298118144065002", "module": "A5"}, {"value": "0", "module": "B1"}, {"value": "35.0766263083994", "module": "B2"}, {"value": "0", "module": "B6"}, {"value": "0", "module": "C1"}, {"value": "0.0679473999805722", "module": "C2"}, {"value": "0.135006170187993", "module": "C3"}, {"value": "2.08593717175035", "module": "C4"}, {"value": "-22.1400688817721", "module": "D"}]}}, {"referenceToLCIAMethodDataSet": {"shortDescription": [{"value": "Incidence of disease due to PM emissions (PM)", "lang": "en"}], "type": "LCIA method data set", "refObjectId": "b5c602c6-def3-11e6-bf01-fe55135034f3", "uri": "../lciamethods/b5c602c6-def3-11e6-bf01-fe55135034f3.xml"}, "other": {"anies": [{"name": "referenceToUnitGroupDataSet", "value": {"shortDescription": [{"value": "Disease incidence", "lang": "en"}], "type": "unit group data set", "refObjectId": "3883559b-648f-4afc-8ba2-0bd24f3affa3", "uri": "../unitgroups/3883559b-648f-4afc-8ba2-0bd24f3affa3.xml"}}, {"value": "2.30225674081581E-05", "module": "A1-A3"}, {"value": "4.44171961562379E-08", "module": "A5"}, {"value": "0", "module": "B1"}, {"value": "2.02910308086189E-06", "module": "B2"}, {"value": "0", "module": "B6"}, {"value": "0", "module": "C1"}, {"value": "1.2098482356483E-07", "module": "C2"}, {"value": "1.07321209820974E-07", "module": "C3"}, {"value": "2.74789829840753E-07", "module": "C4"}, {"value": "-1.23116494874121E-05", "module": "D"}]}}, {"referenceToLCIAMethodDataSet": {"shortDescription": [{"value": "Human exposure efficiency relative to U235 (IR)", "lang": "en"}], "type": "LCIA method data set", "refObjectId": "b5c632be-def3-11e6-bf01-fe55135034f3", "uri": "../lciamethods/b5c632be-def3-11e6-bf01-fe55135034f3.xml"}, "other": {"anies": [{"name": "referenceToUnitGroupDataSet", "value": {"shortDescription": [{"value": "kBq U235-Äq.", "lang": "en"}], "type": "unit group data set", "refObjectId": "456b05bf-1415-44a9-9993-02452f554c09", "uri": "../unitgroups/456b05bf-1415-44a9-9993-02452f554c09.xml"}}, {"value": "11.1343562069571", "module": "A1-A3"}, {"value": "0.0305102012375471", "module": "A5"}, {"value": "0", "module": "B1"}, {"value": "1.36939440046502", "module": "B2"}, {"value": "0", "module": "B6"}, {"value": "0", "module": "C1"}, {"value": "0.0898704464223152", "module": "C2"}, {"value": "0.0867661836735861", "module": "C3"}, {"value": "0.152439806164202", "module": "C4"}, {"value": "-2.57117250943168", "module": "D"}]}}, {"referenceToLCIAMethodDataSet": {"shortDescription": [{"value": "Comparative toxic unit for ecosystems (ETP-fw)", "lang": "en"}], "type": "LCIA method data set", "refObjectId": "ee1082d1-b0f7-43ca-a1f0-21e2a4a74511", "uri": "../lciamethods/ee1082d1-b0f7-43ca-a1f0-21e2a4a74511.xml"}, "other": {"anies": [{"name": "referenceToUnitGroupDataSet", "value": {"shortDescription": [{"value": "CTUe", "lang": "en"}], "type": "unit group data set", "refObjectId": "aa959ded-f1eb-4efb-9c5c-2d60be36b3e6", "uri": "../unitgroups/aa959ded-f1eb-4efb-9c5c-2d60be36b3e6.xml"}}, {"value": "12596.5333540562", "module": "A1-A3"}, {"value": "27.3129755652002", "module": "A5"}, {"value": "0", "module": "B1"}, {"value": "2333.69316482371", "module": "B2"}, {"value": "0", "module": "B6"}, {"value": "0", "module": "C1"}, {"value": "16.3921842656132", "module": "C2"}, {"value": "21.9983797983941", "module": "C3"}, {"value": "503.828343934148", "module": "C4"}, {"value": "-3436.2026823029", "module": "D"}]}}, {"referenceToLCIAMethodDataSet": {"shortDescription": [{"value": "Comparative toxic unit for humans (carcinogenic) (HTP-c)", "lang": "en"}], "type": "LCIA method data set", "refObjectId": "2299222a-bbd8-474f-9d4f-4dd1f18aea7c", "uri": "../lciamethods/2299222a-bbd8-474f-9d4f-4dd1f18aea7c.xml"}, "other": {"anies": [{"name": "referenceToUnitGroupDataSet", "value": {"shortDescription": [{"value": "CTUh", "lang": "en"}], "type": "unit group data set", "refObjectId": "d4c9523e-2d7e-49fd-8469-998f547d3a70", "uri": "../unitgroups/d4c9523e-2d7e-49fd-8469-998f547d3a70.xml"}}, {"value": "1.21072720854916E-06", "module": "A1-A3"}, {"value": "9.24522904707219E-10", "module": "A5"}, {"value": "0", "module": "B1"}, {"value": "1.14435880202678E-07", "module": "B2"}, {"value": "0", "module": "B6"}, {"value": "0", "module": "C1"}, {"value": "6.53801891345088E-10", "module": "C2"}, {"value": "4.94511881532766E-10", "module": "C3"}, {"value": "1.57871508146412E-08", "module": "C4"}, {"value": "-1.71275146216383E-07", "module": "D"}]}}, {"referenceToLCIAMethodDataSet": {"shortDescription": [{"value": "Comparative toxic unit for humans (noncarcinogenic) (HTP-nc)", "lang": "en"}], "type": "LCIA method data set", "refObjectId": "3af763a5-b7a1-48c9-9cee-1f223481fcef", "uri": "../lciamethods/3af763a5-b7a1-48c9-9cee-1f223481fcef.xml"}, "other": {"anies": [{"name": "referenceToUnitGroupDataSet", "value": {"shortDescription": [{"value": "CTUh", "lang": "en"}], "type": "unit group data set", "refObjectId": "d4c9523e-2d7e-49fd-8469-998f547d3a70", "uri": "../unitgroups/d4c9523e-2d7e-49fd-8469-998f547d3a70.xml"}}, {"value": "1.69588510617794E-05", "module": "A1-A3"}, {"value": "1.23559555813168E-08", "module": "A5"}, {"value": "0", "module": "B1"}, {"value": "3.58886191614233E-06", "module": "B2"}, {"value": "0", "module": "B6"}, {"value": "0", "module": "C1"}, {"value": "1.88757163617684E-08", "module": "C2"}, {"value": "2.92757848523121E-08", "module": "C3"}, {"value": "1.81447306147688E-07", "module": "C4"}, {"value": "-2.5314760704938E-06", "module": "D"}]}}, {"referenceToLCIAMethodDataSet": {"shortDescription": [{"value": "Soil quality index (SQP)", "lang": "en"}], "type": "LCIA method data set", "refObjectId": "b2ad6890-c78d-11e6-9d9d-cec0c932ce01", "uri": "../lciamethods/b2ad6890-c78d-11e6-9d9d-cec0c932ce01.xml"}, "other": {"anies": [{"name": "referenceToUnitGroupDataSet", "value": {"shortDescription": [{"value": "SQP", "lang": "en"}], "type": "unit group data set", "refObjectId": "f130951c-e67f-4f7f-8dd4-665de3974e18", "uri": "../unitgroups/f130951c-e67f-4f7f-8dd4-665de3974e18.xml"}}, {"value": "2353.17003309922", "module": "A1-A3"}, {"value": "5.97681595506458", "module": "A5"}, {"value": "0", "module": "B1"}, {"value": "169.293906161355", "module": "B2"}, {"value": "0", "module": "B6"}, {"value": "0", "module": "C1"}, {"value": "17.6590641896623", "module": "C2"}, {"value": "3.63315859010175", "module": "C3"}, {"value": "27.3383567122675", "module": "C4"}, {"value": "-251.664740829159", "module": "D"}]}}]}, "otherAttributes": {"{http://www.indata.network/EPD/2019}epd-version": "1.2"}, "version": "1.1", "locations": "../ILCDLocations.xml"}