{"processInformation": {"dataSetInformation": {"UUID": "f6fbb446-db01-47e1-93f3-375d77f4cf37", "name": {"baseName": [{"value": "Surface temperature control - Viega - Fonterra control system", "lang": "en"}, {"value": "Flächentemperierung - Viega - Fonterra Regelung", "lang": "de"}]}, "classificationInformation": {"classification": [{"class": [{"value": "Gebäudetechnik", "level": 0, "classId": "8"}, {"value": "Sanitär", "level": 1, "classId": "8.3"}, {"value": "Armaturen", "level": 2, "classId": "8.3.02"}], "name": "OEKOBAU.DAT"}]}, "generalComment": [{"value": "Dieser Datensatz beinhaltet die Ergebnisse für die Module A1-A3 sowie Module A4, A5, B1, B2, B3, B4, B5, B6, B7, C1, C2, C3, C4, D. Das Umweltprofil beinhaltet die Aufwendungen für die Lebenszyklus-Stadien cradle to grave (Modul A + B + C + D). Die Herstellung der Verpackung wurde innerhalb der Module A1-A3 berücksichtigt.", "lang": "de"}, {"value": "This data set contains the results for modules A1-A3 and modules A4, A5, B1, B2, B3, B4, B5, B6, B7, C1, C2, C3, C4, D. The environmental profile contains the expenditure for the cradle to grave life cycle stages (modules A + B + C + D). The production of the packaging was taken into account within modules A1-A3.", "lang": "en"}], "other": {"anies": [{"margins": 0.0}, "<ns11:modules xmlns:ns11=\"http://openlca.org/epd_ilcd\" xmlns=\"http://lca.jrc.it/ILCD/Process\" xmlns:c=\"http://lca.jrc.it/ILCD/Contact\" xmlns:common=\"http://lca.jrc.it/ILCD/Common\" xmlns:epd=\"http://www.iai.kit.edu/EPD/2013\" xmlns:epd2=\"http://www.indata.network/EPD/2019\" xmlns:f=\"http://lca.jrc.it/ILCD/Flow\" xmlns:fp=\"http://lca.jrc.it/ILCD/FlowProperty\" xmlns:m=\"http://lca.jrc.it/ILCD/LCIAMethod\" xmlns:ns9=\"http://www.okworx.com/ILCD/Extensions/2018/Profile\" xmlns:s=\"http://lca.jrc.it/ILCD/Source\" xmlns:u=\"http://lca.jrc.it/ILCD/UnitGroup\" name=\"A1-A3\"/>", "<ns11:modules xmlns:ns11=\"http://openlca.org/epd_ilcd\" xmlns=\"http://lca.jrc.it/ILCD/Process\" xmlns:c=\"http://lca.jrc.it/ILCD/Contact\" xmlns:common=\"http://lca.jrc.it/ILCD/Common\" xmlns:epd=\"http://www.iai.kit.edu/EPD/2013\" xmlns:epd2=\"http://www.indata.network/EPD/2019\" xmlns:f=\"http://lca.jrc.it/ILCD/Flow\" xmlns:fp=\"http://lca.jrc.it/ILCD/FlowProperty\" xmlns:m=\"http://lca.jrc.it/ILCD/LCIAMethod\" xmlns:ns9=\"http://www.okworx.com/ILCD/Extensions/2018/Profile\" xmlns:s=\"http://lca.jrc.it/ILCD/Source\" xmlns:u=\"http://lca.jrc.it/ILCD/UnitGroup\" name=\"A4\"/>", "<ns11:modules xmlns:ns11=\"http://openlca.org/epd_ilcd\" xmlns=\"http://lca.jrc.it/ILCD/Process\" xmlns:c=\"http://lca.jrc.it/ILCD/Contact\" xmlns:common=\"http://lca.jrc.it/ILCD/Common\" xmlns:epd=\"http://www.iai.kit.edu/EPD/2013\" xmlns:epd2=\"http://www.indata.network/EPD/2019\" xmlns:f=\"http://lca.jrc.it/ILCD/Flow\" xmlns:fp=\"http://lca.jrc.it/ILCD/FlowProperty\" xmlns:m=\"http://lca.jrc.it/ILCD/LCIAMethod\" xmlns:ns9=\"http://www.okworx.com/ILCD/Extensions/2018/Profile\" xmlns:s=\"http://lca.jrc.it/ILCD/Source\" xmlns:u=\"http://lca.jrc.it/ILCD/UnitGroup\" name=\"A5\"/>", "<ns11:modules xmlns:ns11=\"http://openlca.org/epd_ilcd\" xmlns=\"http://lca.jrc.it/ILCD/Process\" xmlns:c=\"http://lca.jrc.it/ILCD/Contact\" xmlns:common=\"http://lca.jrc.it/ILCD/Common\" xmlns:epd=\"http://www.iai.kit.edu/EPD/2013\" xmlns:epd2=\"http://www.indata.network/EPD/2019\" xmlns:f=\"http://lca.jrc.it/ILCD/Flow\" xmlns:fp=\"http://lca.jrc.it/ILCD/FlowProperty\" xmlns:m=\"http://lca.jrc.it/ILCD/LCIAMethod\" xmlns:ns9=\"http://www.okworx.com/ILCD/Extensions/2018/Profile\" xmlns:s=\"http://lca.jrc.it/ILCD/Source\" xmlns:u=\"http://lca.jrc.it/ILCD/UnitGroup\" name=\"B1\"/>", "<ns11:modules xmlns:ns11=\"http://openlca.org/epd_ilcd\" xmlns=\"http://lca.jrc.it/ILCD/Process\" xmlns:c=\"http://lca.jrc.it/ILCD/Contact\" xmlns:common=\"http://lca.jrc.it/ILCD/Common\" xmlns:epd=\"http://www.iai.kit.edu/EPD/2013\" xmlns:epd2=\"http://www.indata.network/EPD/2019\" xmlns:f=\"http://lca.jrc.it/ILCD/Flow\" xmlns:fp=\"http://lca.jrc.it/ILCD/FlowProperty\" xmlns:m=\"http://lca.jrc.it/ILCD/LCIAMethod\" xmlns:ns9=\"http://www.okworx.com/ILCD/Extensions/2018/Profile\" xmlns:s=\"http://lca.jrc.it/ILCD/Source\" xmlns:u=\"http://lca.jrc.it/ILCD/UnitGroup\" name=\"B2\"/>", "<ns11:modules xmlns:ns11=\"http://openlca.org/epd_ilcd\" xmlns=\"http://lca.jrc.it/ILCD/Process\" xmlns:c=\"http://lca.jrc.it/ILCD/Contact\" xmlns:common=\"http://lca.jrc.it/ILCD/Common\" xmlns:epd=\"http://www.iai.kit.edu/EPD/2013\" xmlns:epd2=\"http://www.indata.network/EPD/2019\" xmlns:f=\"http://lca.jrc.it/ILCD/Flow\" xmlns:fp=\"http://lca.jrc.it/ILCD/FlowProperty\" xmlns:m=\"http://lca.jrc.it/ILCD/LCIAMethod\" xmlns:ns9=\"http://www.okworx.com/ILCD/Extensions/2018/Profile\" xmlns:s=\"http://lca.jrc.it/ILCD/Source\" xmlns:u=\"http://lca.jrc.it/ILCD/UnitGroup\" name=\"B3\"/>", "<ns11:modules xmlns:ns11=\"http://openlca.org/epd_ilcd\" xmlns=\"http://lca.jrc.it/ILCD/Process\" xmlns:c=\"http://lca.jrc.it/ILCD/Contact\" xmlns:common=\"http://lca.jrc.it/ILCD/Common\" xmlns:epd=\"http://www.iai.kit.edu/EPD/2013\" xmlns:epd2=\"http://www.indata.network/EPD/2019\" xmlns:f=\"http://lca.jrc.it/ILCD/Flow\" xmlns:fp=\"http://lca.jrc.it/ILCD/FlowProperty\" xmlns:m=\"http://lca.jrc.it/ILCD/LCIAMethod\" xmlns:ns9=\"http://www.okworx.com/ILCD/Extensions/2018/Profile\" xmlns:s=\"http://lca.jrc.it/ILCD/Source\" xmlns:u=\"http://lca.jrc.it/ILCD/UnitGroup\" name=\"B4\"/>", "<ns11:modules xmlns:ns11=\"http://openlca.org/epd_ilcd\" xmlns=\"http://lca.jrc.it/ILCD/Process\" xmlns:c=\"http://lca.jrc.it/ILCD/Contact\" xmlns:common=\"http://lca.jrc.it/ILCD/Common\" xmlns:epd=\"http://www.iai.kit.edu/EPD/2013\" xmlns:epd2=\"http://www.indata.network/EPD/2019\" xmlns:f=\"http://lca.jrc.it/ILCD/Flow\" xmlns:fp=\"http://lca.jrc.it/ILCD/FlowProperty\" xmlns:m=\"http://lca.jrc.it/ILCD/LCIAMethod\" xmlns:ns9=\"http://www.okworx.com/ILCD/Extensions/2018/Profile\" xmlns:s=\"http://lca.jrc.it/ILCD/Source\" xmlns:u=\"http://lca.jrc.it/ILCD/UnitGroup\" name=\"B5\"/>", "<ns11:modules xmlns:ns11=\"http://openlca.org/epd_ilcd\" xmlns=\"http://lca.jrc.it/ILCD/Process\" xmlns:c=\"http://lca.jrc.it/ILCD/Contact\" xmlns:common=\"http://lca.jrc.it/ILCD/Common\" xmlns:epd=\"http://www.iai.kit.edu/EPD/2013\" xmlns:epd2=\"http://www.indata.network/EPD/2019\" xmlns:f=\"http://lca.jrc.it/ILCD/Flow\" xmlns:fp=\"http://lca.jrc.it/ILCD/FlowProperty\" xmlns:m=\"http://lca.jrc.it/ILCD/LCIAMethod\" xmlns:ns9=\"http://www.okworx.com/ILCD/Extensions/2018/Profile\" xmlns:s=\"http://lca.jrc.it/ILCD/Source\" xmlns:u=\"http://lca.jrc.it/ILCD/UnitGroup\" name=\"B6\"/>", "<ns11:modules xmlns:ns11=\"http://openlca.org/epd_ilcd\" xmlns=\"http://lca.jrc.it/ILCD/Process\" xmlns:c=\"http://lca.jrc.it/ILCD/Contact\" xmlns:common=\"http://lca.jrc.it/ILCD/Common\" xmlns:epd=\"http://www.iai.kit.edu/EPD/2013\" xmlns:epd2=\"http://www.indata.network/EPD/2019\" xmlns:f=\"http://lca.jrc.it/ILCD/Flow\" xmlns:fp=\"http://lca.jrc.it/ILCD/FlowProperty\" xmlns:m=\"http://lca.jrc.it/ILCD/LCIAMethod\" xmlns:ns9=\"http://www.okworx.com/ILCD/Extensions/2018/Profile\" xmlns:s=\"http://lca.jrc.it/ILCD/Source\" xmlns:u=\"http://lca.jrc.it/ILCD/UnitGroup\" name=\"B7\"/>", "<ns11:modules xmlns:ns11=\"http://openlca.org/epd_ilcd\" xmlns=\"http://lca.jrc.it/ILCD/Process\" xmlns:c=\"http://lca.jrc.it/ILCD/Contact\" xmlns:common=\"http://lca.jrc.it/ILCD/Common\" xmlns:epd=\"http://www.iai.kit.edu/EPD/2013\" xmlns:epd2=\"http://www.indata.network/EPD/2019\" xmlns:f=\"http://lca.jrc.it/ILCD/Flow\" xmlns:fp=\"http://lca.jrc.it/ILCD/FlowProperty\" xmlns:m=\"http://lca.jrc.it/ILCD/LCIAMethod\" xmlns:ns9=\"http://www.okworx.com/ILCD/Extensions/2018/Profile\" xmlns:s=\"http://lca.jrc.it/ILCD/Source\" xmlns:u=\"http://lca.jrc.it/ILCD/UnitGroup\" name=\"C1\"/>", "<ns11:modules xmlns:ns11=\"http://openlca.org/epd_ilcd\" xmlns=\"http://lca.jrc.it/ILCD/Process\" xmlns:c=\"http://lca.jrc.it/ILCD/Contact\" xmlns:common=\"http://lca.jrc.it/ILCD/Common\" xmlns:epd=\"http://www.iai.kit.edu/EPD/2013\" xmlns:epd2=\"http://www.indata.network/EPD/2019\" xmlns:f=\"http://lca.jrc.it/ILCD/Flow\" xmlns:fp=\"http://lca.jrc.it/ILCD/FlowProperty\" xmlns:m=\"http://lca.jrc.it/ILCD/LCIAMethod\" xmlns:ns9=\"http://www.okworx.com/ILCD/Extensions/2018/Profile\" xmlns:s=\"http://lca.jrc.it/ILCD/Source\" xmlns:u=\"http://lca.jrc.it/ILCD/UnitGroup\" name=\"C2\"/>", "<ns11:modules xmlns:ns11=\"http://openlca.org/epd_ilcd\" xmlns=\"http://lca.jrc.it/ILCD/Process\" xmlns:c=\"http://lca.jrc.it/ILCD/Contact\" xmlns:common=\"http://lca.jrc.it/ILCD/Common\" xmlns:epd=\"http://www.iai.kit.edu/EPD/2013\" xmlns:epd2=\"http://www.indata.network/EPD/2019\" xmlns:f=\"http://lca.jrc.it/ILCD/Flow\" xmlns:fp=\"http://lca.jrc.it/ILCD/FlowProperty\" xmlns:m=\"http://lca.jrc.it/ILCD/LCIAMethod\" xmlns:ns9=\"http://www.okworx.com/ILCD/Extensions/2018/Profile\" xmlns:s=\"http://lca.jrc.it/ILCD/Source\" xmlns:u=\"http://lca.jrc.it/ILCD/UnitGroup\" name=\"C3\"/>", "<ns11:modules xmlns:ns11=\"http://openlca.org/epd_ilcd\" xmlns=\"http://lca.jrc.it/ILCD/Process\" xmlns:c=\"http://lca.jrc.it/ILCD/Contact\" xmlns:common=\"http://lca.jrc.it/ILCD/Common\" xmlns:epd=\"http://www.iai.kit.edu/EPD/2013\" xmlns:epd2=\"http://www.indata.network/EPD/2019\" xmlns:f=\"http://lca.jrc.it/ILCD/Flow\" xmlns:fp=\"http://lca.jrc.it/ILCD/FlowProperty\" xmlns:m=\"http://lca.jrc.it/ILCD/LCIAMethod\" xmlns:ns9=\"http://www.okworx.com/ILCD/Extensions/2018/Profile\" xmlns:s=\"http://lca.jrc.it/ILCD/Source\" xmlns:u=\"http://lca.jrc.it/ILCD/UnitGroup\" name=\"C4\"/>", "<ns11:modules xmlns:ns11=\"http://openlca.org/epd_ilcd\" xmlns=\"http://lca.jrc.it/ILCD/Process\" xmlns:c=\"http://lca.jrc.it/ILCD/Contact\" xmlns:common=\"http://lca.jrc.it/ILCD/Common\" xmlns:epd=\"http://www.iai.kit.edu/EPD/2013\" xmlns:epd2=\"http://www.indata.network/EPD/2019\" xmlns:f=\"http://lca.jrc.it/ILCD/Flow\" xmlns:fp=\"http://lca.jrc.it/ILCD/FlowProperty\" xmlns:m=\"http://lca.jrc.it/ILCD/LCIAMethod\" xmlns:ns9=\"http://www.okworx.com/ILCD/Extensions/2018/Profile\" xmlns:s=\"http://lca.jrc.it/ILCD/Source\" xmlns:u=\"http://lca.jrc.it/ILCD/UnitGroup\" name=\"D\"/>"]}}, "quantitativeReference": {"referenceToReferenceFlow": [1], "type": "Reference flow(s)"}, "time": {"referenceYear": 2024, "dataSetValidUntil": 2029, "timeRepresentativenessDescription": [{"value": "jährlicher Durchschnitt", "lang": "de"}, {"value": "annual average", "lang": "en"}], "other": {"anies": [{"name": "publicationDateOfEPD", "value": 1727740800000}]}}, "geography": {"locationOfOperationSupplyOrProduction": {"descriptionOfRestrictions": [{"value": "Dieser Datensatz repräsentiert die Situation des Unternehmens Viega GmbH & Co. KG, Niederwinkling und Ennest  im Hinblick auf die wichtigsten Technologien und die gesetzlichen Rahmenbedingungen.", "lang": "de"}, {"value": "This data set represents the situation of Viega GmbH & Co. KG, Niederwinkling and Ennest with regard to the most important technologies and the legal framework.", "lang": "en"}], "location": "DE"}}, "technology": {"technologyDescriptionAndIncludedProcesses": [{"value": "Die Ökobilanzergebnisse umfassen die Lebenszyklusstadien der Herstellung der Vorprodukte bis hin zur Rohstoffgewinnung und Verarbeitungsprozesse von als Input dienenden Sekundärstoffen (z.B. Recyclingprozesse), deren Transporte zum Werk sowie die Produktion selbst, einschließlich der Bereitstellung von allen Hilfs- und Betriebsstoffen, Energie, sowie die vollständige Abfallbehandlung oder die Deponierung der Restabfälle während des Stadiums der Produktion. Die Module A1, A2 und A3 sind hier als ein aggregiertes Modul A1-A3 ausgewiesen. Falls für diesen Datensatz weitere Module berechnet wurden, sind diese separat zu finden und können für eine Betrachtung des gesamten Lebenszyklus zusammengeführt werden.", "lang": "de"}, {"value": "The life cycle assessment results cover the life cycle stages of manufacturing the intermediate products up to raw material extraction and processing operations of secondary materials serving as input (e.g. recycling processes), their transports to the plant as well as the production itself, including the provision of all auxiliary and operating materials, energy, and the complete waste treatment or landfilling of the residual waste during the stage of production. Modules A1, A2, and A3 are shown here as one aggregated module A1-A3. If further modules were calculated for this data set, they can be found separately and can be combined for a consideration of the entire life cycle.", "lang": "en"}], "technologicalApplicability": [{"value": "Fonterra-Flächentemperiersysteme für das Beheizen und Kühlen von Räumen.", "lang": "de"}, {"value": "Fonterra surface temperature control systems for heating and cooling rooms.", "lang": "en"}]}}, "modellingAndValidation": {"LCIMethodAndAllocation": {"typeOfDataSet": "EPD", "referenceToLCAMethodDetails": [{"shortDescription": [{"value": "Produktkategorieregeln Teil A", "lang": "de"}, {"value": "Product category rules Part A", "lang": "en"}], "type": "source data set", "refObjectId": "c6e986be-62a9-4f2f-b486-27aa9129eaeb", "version": "00.00.014"}, {"shortDescription": [{"value": "Produktkategorieregeln Teil B – für Flächentemperierungssysteme und Zubehör", "lang": "de"}, {"value": "Product category rules Part B – for surface tempering systems und accessories", "lang": "en"}], "type": "source data set", "refObjectId": "c412790b-2fe8-4a04-a71e-ebd32d7ead07", "version": "00.00.005"}], "other": {"anies": [{"name": "subType", "value": "average dataset"}]}}, "dataSourcesTreatmentAndRepresentativeness": {"referenceToDataSource": [{"shortDescription": [{"value": "ecoinvent database (general)", "lang": "en"}], "type": "source data set", "refObjectId": "b497a91f-e14b-4b69-8f28-f50eb1576766", "version": "00.03.002"}], "useAdviceForDataSet": [{"value": "Dieser Datensatz beinhaltet die Ergebnisse für die Module A1-A3 sowie die Module A4, A5, B1, B2, B3, B4, B5, B6, B7, C1, C2, C3, C4 und D gemäß EN 15804 + A2.\r\nDie Modellierung der B-Module wurde bezogen auf 1 Jahr vorgenommen.\r\nEin Vergleich mit anderen Produkten ist nur mit einer vergleichbaren Anwendung im Gebäude zulässig. Grundsätzlich ist eine Gegenüberstellung oder die Bewertung von EPD Daten nur möglich, wenn alle zu vergleichenden Datensätze nach EN 15804 + A2 erstellt wurden und der Gebäudekontext, bzw. die produktspezifischen Leistungsmerkmale berücksichtigt werden.", "lang": "de"}], "other": {"anies": [{"name": "referenceToOriginalEPD", "value": {"shortDescription": {"value": "EPD Flächentemperierung - Viega - Fonterra", "defaultValue": "EPD Flächentemperierung - Viega - Fonterra", "lstrings": [{"lang": "de", "value": "EPD Flächentemperierung - Viega - Fonterra"}]}, "version": {"version": 2, "majorVersion": 0, "minorVersion": 0, "subMinorVersion": 2, "zero": false, "versionString": "00.00.002"}, "type": "source data set", "uuid": {"uuid": "b6e892e8-8100-4b91-b594-f6d454fe45f3"}, "refObjectId": "b6e892e8-8100-4b91-b594-f6d454fe45f3", "versionAsString": "00.00.002", "resourceURLs": ["https://oekobaudat.de/OEKOBAU.DAT/resource/sources/b6e892e8-8100-4b91-b594-f6d454fe45f3/EPD-VFT-GB-67.0_v4.pdf?version=00.00.002", "https://oekobaudat.de/OEKOBAU.DAT/resource/sources/b6e892e8-8100-4b91-b594-f6d454fe45f3/EPD-VFT-67.0_v4.pdf?version=00.00.002"]}}]}}, "validation": {"review": [{"reviewDetails": [{"value": "Die angewendete LCI Methode ist in Übereinstimmung mit ISO 14040 und 14044. Die Dokumentation enthält alle relevanten Informationen im Hinblick auf die Datenqualität und den Umfang der Anwendung der jeweiligen LCI Ergebnisse bzw. der Datensätze. Der Datensatz repräsentiert den Stand der Technik bezogen auf die funktionelle Einheit.", "lang": "de"}], "referenceToNameOfReviewerAndInstitution": [{"shortDescription": [{"value": "Eric Brehm", "lang": "de"}], "type": "contact data set", "refObjectId": "ef2baa7d-04f8-424a-af3d-38561f10b8d1", "version": "00.00.001"}], "type": "Independent external review"}]}, "complianceDeclarations": {"compliance": [{"referenceToComplianceSystem": {"shortDescription": [{"value": "EN 15804+A2 (EF 3.0)", "lang": "de"}, {"value": "EN 15804+A2 (EF 3.0)", "lang": "en"}], "type": "source data set", "refObjectId": "c0016b33-8cf7-415c-ac6e-deba0d21440d", "version": "00.02.000"}}]}}, "administrativeInformation": {"dataGenerator": {"referenceToPersonOrEntityGeneratingTheDataSet": [{"shortDescription": [{"value": "Viega GmbH & Co. KG", "lang": "de"}], "type": "contact data set", "refObjectId": "6641b025-d17c-4a22-ab87-168a1be6722b", "version": "00.00.001"}]}, "dataEntryBy": {"timeStamp": 1756733640929, "referenceToDataSetFormat": [{"shortDescription": [{"value": "EPD Data Format Extensions v1.2", "lang": "en"}, {"value": "EPD-Datenformaterweiterungen v1.2", "lang": "de"}], "type": "source data set", "refObjectId": "a29449fd-aa2f-4de8-b5d7-4b06b43c6fde", "version": "00.01.003"}, {"shortDescription": [{"value": "ILCD format", "lang": "en"}], "type": "source data set", "refObjectId": "a97a0155-0234-4b87-b4ce-a45da52f2a40", "version": "03.01.004", "uri": "http://lca.jrc.ec.europa.eu/lcainfohub/datasets/ilcd/sources/a97a0155-0234-4b87-b4ce-a45da52f2a40.xml"}], "referenceToPersonOrEntityEnteringTheData": {"shortDescription": [{"value": "ift Rosenheim", "lang": "de"}], "type": "contact data set", "refObjectId": "bdf65bd4-c474-4c23-8269-124ba43fa2b9", "version": "25.00.004"}}, "publicationAndOwnership": {"dataSetVersion": "00.00.013", "referenceToRegistrationAuthority": {"shortDescription": [{"value": "ift Rosenheim", "lang": "de"}], "type": "contact data set", "refObjectId": "bdf65bd4-c474-4c23-8269-124ba43fa2b9", "version": "25.00.004"}, "registrationNumber": "EPD-VFT-67.0", "referenceToOwnershipOfDataSet": {"shortDescription": [{"value": "Viega GmbH & Co. KG", "lang": "de"}], "type": "contact data set", "refObjectId": "6641b025-d17c-4a22-ab87-168a1be6722b", "version": "00.00.001"}, "copyright": true, "licenseType": "Free of charge for all users and uses", "accessRestrictions": [{"value": "none", "lang": "de"}], "other": {"anies": [{"name": "referenceToPublisher", "value": {"shortDescription": [{"value": "ift Rosenheim", "lang": "de"}], "type": "contact data set", "refObjectId": "bdf65bd4-c474-4c23-8269-124ba43fa2b9", "version": "25.00.004"}}]}}}, "exchanges": {"exchange": [{"dataSetInternalID": 1, "referenceToFlowDataSet": {"shortDescription": [{"value": "Flächentemperierung - Viega - Fonterra Regelung", "lang": "de"}], "type": "flow data set", "refObjectId": "4b49ab23-8c44-44da-afba-3401464b73df", "version": "00.00.005"}, "meanAmount": 1.0, "resultingAmount": 1.0, "referenceFlow": true, "resultingflowAmount": 1.0, "flowProperties": [{"name": [{"lang": "de", "value": "Anzahl"}, {"lang": "en", "value": "Number of pieces"}], "uuid": "01846770-4cfe-4a25-8ad9-919d8d378345", "referenceFlowProperty": true, "meanValue": 1.0, "referenceUnit": "pcs.", "unitGroupUUID": "934110e3-baf4-49e9-992c-3d8109a6aafb"}, {"name": [{"lang": "de", "value": "Biogener Kohlenstoffgehalt in der zugehörigen Verpackung (Biog. C in packaging)"}, {"lang": "en", "value": "Biogenic carbon content in accompanying packaging (Biog. C in packaging)"}], "uuid": "262a541b-209e-44cc-a426-33bce30de7b1", "meanValue": 0.092}, {"name": [{"lang": "de", "value": "Biogener Kohlenstoffgehalt im Produkt (Biog. C in product)"}, {"lang": "en", "value": "Biogenic carbon content in product (Biog. C in product)"}], "uuid": "62e503ce-544a-4599-b2ad-bcea15a7bf20", "meanValue": 0.0}], "materialProperties": [{"name": "weight per piece", "value": "1.04", "unit": "kg"}], "typeOfFlow": "Product flow", "classification": {"classHierarchy": "Gebäudetechnik / Sanitär / Armaturen", "name": "OEKOBAU.DAT"}}, {"dataSetInternalID": 2, "referenceToFlowDataSet": {"shortDescription": [{"value": "Components for re-use (CRU)", "lang": "en"}, {"value": "Komponenten für die Wiederverwendung (CRU)", "lang": "de"}], "type": "flow data set", "refObjectId": "a2b32f97-3fc7-4af2-b209-525bc6426f33", "version": "38.00.000"}, "exchange direction": "OUTPUT", "meanAmount": 0.0, "other": {"anies": [{"value": "0.0", "module": "A1-A3"}, {"value": "0.0", "module": "A4"}, {"value": "0.0", "module": "A5"}, {"value": "0.0", "module": "B1"}, {"value": "0.0", "module": "B2"}, {"value": "0.0", "module": "B3"}, {"value": "0.0", "module": "B4"}, {"value": "0.0", "module": "B5"}, {"value": "0.0", "module": "B6"}, {"value": "0.0", "module": "B7"}, {"value": "0.0", "module": "C1"}, {"value": "0.0", "module": "C2"}, {"value": "0.0", "module": "C3"}, {"value": "0.0", "module": "C4"}, {"value": "0.0", "module": "D"}, {"name": "referenceToUnitGroupDataSet", "value": {"shortDescription": [{"value": "kg"}], "type": "unit group data set", "refObjectId": "ad38d542-3fe9-439d-9b95-2f5f7752acaf", "uri": "../unitgroups/ad38d542-3fe9-439d-9b95-2f5f7752acaf"}}]}, "flowProperties": [], "typeOfFlow": "Other flow", "classification": {"classHierarchy": "Quantities / Environmental quantities / EPD EN 15804 / LCI indicators", "name": "GaBiCategories"}}, {"dataSetInternalID": 3, "referenceToFlowDataSet": {"shortDescription": [{"value": "Exported electrical energy (EEE)", "lang": "en"}, {"value": "Exportierte elektrische Energie (EEE)", "lang": "de"}], "type": "flow data set", "refObjectId": "4da0c987-2b76-40d6-9e9e-82a017aaaf29", "version": "38.00.000"}, "exchange direction": "OUTPUT", "meanAmount": 0.0, "other": {"anies": [{"value": "1.56", "module": "A1-A3"}, {"value": "1.82E-4", "module": "A4"}, {"value": "6.05E-6", "module": "A5"}, {"value": "0.0", "module": "B1"}, {"value": "0.0", "module": "B2"}, {"value": "0.0", "module": "B3"}, {"value": "0.0", "module": "B4"}, {"value": "0.0", "module": "B5"}, {"value": "7.24", "module": "B6"}, {"value": "0.0", "module": "B7"}, {"value": "1.04E-6", "module": "C1"}, {"value": "1.32E-5", "module": "C2"}, {"value": "2.03E-4", "module": "C3"}, {"value": "9.7E-6", "module": "C4"}, {"value": "-0.21", "module": "D"}, {"name": "referenceToUnitGroupDataSet", "value": {"shortDescription": [{"value": "MJ"}], "type": "unit group data set", "refObjectId": "93a60a57-a3c8-11da-a746-0800200c9a66", "uri": "../unitgroups/93a60a57-a3c8-11da-a746-0800200c9a66"}}]}, "flowProperties": [], "typeOfFlow": "Other flow", "classification": {"classHierarchy": "Quantities / Environmental quantities / EPD EN 15804 / LCI indicators", "name": "GaBiCategories"}}, {"dataSetInternalID": 4, "referenceToFlowDataSet": {"shortDescription": [{"value": "Exported thermal energy (EET)", "lang": "en"}, {"value": "Exportierte thermische Energie (EET)", "lang": "de"}], "type": "flow data set", "refObjectId": "98daf38a-7a79-46d3-9a37-2b7bd0955810", "version": "38.00.000"}, "exchange direction": "OUTPUT", "meanAmount": 0.0, "other": {"anies": [{"value": "0.0", "module": "A1-A3"}, {"value": "0.0", "module": "A4"}, {"value": "0.0", "module": "A5"}, {"value": "0.0", "module": "B1"}, {"value": "0.0", "module": "B2"}, {"value": "0.0", "module": "B3"}, {"value": "0.0", "module": "B4"}, {"value": "0.0", "module": "B5"}, {"value": "0.0", "module": "B6"}, {"value": "0.0", "module": "B7"}, {"value": "0.0", "module": "C1"}, {"value": "0.0", "module": "C2"}, {"value": "0.0", "module": "C3"}, {"value": "0.0", "module": "C4"}, {"value": "0.0", "module": "D"}, {"name": "referenceToUnitGroupDataSet", "value": {"shortDescription": [{"value": "MJ"}], "type": "unit group data set", "refObjectId": "93a60a57-a3c8-11da-a746-0800200c9a66", "uri": "../unitgroups/93a60a57-a3c8-11da-a746-0800200c9a66"}}]}, "flowProperties": [], "typeOfFlow": "Other flow", "classification": {"classHierarchy": "Quantities / Environmental quantities / EPD EN 15804 / LCI indicators", "name": "GaBiCategories"}}, {"dataSetInternalID": 5, "referenceToFlowDataSet": {"shortDescription": [{"value": "Hazardous waste disposed (HWD)", "lang": "en"}, {"value": "Gefährlicher Abfall zur Beseitigung (HWD)", "lang": "de"}], "type": "flow data set", "refObjectId": "430f9e0f-59b2-46a0-8e0d-55e0e84948fc", "version": "38.00.000"}, "exchange direction": "OUTPUT", "meanAmount": 0.0, "other": {"anies": [{"value": "9.94", "module": "A1-A3"}, {"value": "0.0017", "module": "A4"}, {"value": "3.22E-4", "module": "A5"}, {"value": "0.0", "module": "B1"}, {"value": "0.0", "module": "B2"}, {"value": "0.0", "module": "B3"}, {"value": "0.0", "module": "B4"}, {"value": "0.0", "module": "B5"}, {"value": "3.96", "module": "B6"}, {"value": "0.0", "module": "B7"}, {"value": "8.33E-6", "module": "C1"}, {"value": "1.23E-4", "module": "C2"}, {"value": "0.00155", "module": "C3"}, {"value": "7.77E-5", "module": "C4"}, {"value": "-2.0", "module": "D"}, {"name": "referenceToUnitGroupDataSet", "value": {"shortDescription": [{"value": "kg"}], "type": "unit group data set", "refObjectId": "ad38d542-3fe9-439d-9b95-2f5f7752acaf", "uri": "../unitgroups/ad38d542-3fe9-439d-9b95-2f5f7752acaf"}}]}, "flowProperties": [], "typeOfFlow": "Other flow", "classification": {"classHierarchy": "Quantities / Environmental quantities / EPD EN 15804 / LCI indicators", "name": "GaBiCategories"}}, {"dataSetInternalID": 6, "referenceToFlowDataSet": {"shortDescription": [{"value": "Material for Energy Recovery (MER)", "lang": "en"}, {"value": "Stoff für die Energierückgewinnung (MER)", "lang": "de"}], "type": "flow data set", "refObjectId": "59a9181c-3aaf-46ee-8b13-2b3723b6e447", "version": "38.00.000"}, "exchange direction": "OUTPUT", "meanAmount": 0.0, "other": {"anies": [{"value": "3.37E-4", "module": "A1-A3"}, {"value": "4.61E-8", "module": "A4"}, {"value": "1.64E-9", "module": "A5"}, {"value": "0.0", "module": "B1"}, {"value": "0.0", "module": "B2"}, {"value": "0.0", "module": "B3"}, {"value": "0.0", "module": "B4"}, {"value": "0.0", "module": "B5"}, {"value": "2.19E-5", "module": "B6"}, {"value": "0.0", "module": "B7"}, {"value": "2.03E-10", "module": "C1"}, {"value": "3.22E-9", "module": "C2"}, {"value": "1.96E-8", "module": "C3"}, {"value": "1.9E-9", "module": "C4"}, {"value": "-2.89E-5", "module": "D"}, {"name": "referenceToUnitGroupDataSet", "value": {"shortDescription": [{"value": "kg"}], "type": "unit group data set", "refObjectId": "ad38d542-3fe9-439d-9b95-2f5f7752acaf", "uri": "../unitgroups/ad38d542-3fe9-439d-9b95-2f5f7752acaf"}}]}, "flowProperties": [], "typeOfFlow": "Other flow", "classification": {"classHierarchy": "Quantities / Environmental quantities / EPD EN 15804 / LCI indicators", "name": "GaBiCategories"}}, {"dataSetInternalID": 7, "referenceToFlowDataSet": {"shortDescription": [{"value": "Materials for Recycling (MFR)", "lang": "en"}, {"value": "Stoffe zum Recycling (MFR)", "lang": "de"}], "type": "flow data set", "refObjectId": "d7fe48a5-4103-49c8-9aae-b0b5dfdbd6ae", "version": "38.00.000"}, "exchange direction": "OUTPUT", "meanAmount": 0.0, "other": {"anies": [{"value": "0.0586", "module": "A1-A3"}, {"value": "7.5E-6", "module": "A4"}, {"value": "1.92E-7", "module": "A5"}, {"value": "0.0", "module": "B1"}, {"value": "0.0", "module": "B2"}, {"value": "0.0", "module": "B3"}, {"value": "0.0", "module": "B4"}, {"value": "0.0", "module": "B5"}, {"value": "0.16", "module": "B6"}, {"value": "0.0", "module": "B7"}, {"value": "5.87E-8", "module": "C1"}, {"value": "5.42E-7", "module": "C2"}, {"value": "0.0999", "module": "C3"}, {"value": "5.47E-7", "module": "C4"}, {"value": "-0.014", "module": "D"}, {"name": "referenceToUnitGroupDataSet", "value": {"shortDescription": [{"value": "kg"}], "type": "unit group data set", "refObjectId": "ad38d542-3fe9-439d-9b95-2f5f7752acaf", "uri": "../unitgroups/ad38d542-3fe9-439d-9b95-2f5f7752acaf"}}]}, "flowProperties": [], "typeOfFlow": "Other flow", "classification": {"classHierarchy": "Quantities / Environmental quantities / EPD EN 15804 / LCI indicators", "name": "GaBiCategories"}}, {"dataSetInternalID": 8, "referenceToFlowDataSet": {"shortDescription": [{"value": "Use of net fresh water (FW)", "lang": "en"}, {"value": "Frischwasserverbrauch (FW)", "lang": "de"}], "type": "flow data set", "refObjectId": "3cf952c8-f3a4-461d-8c96-96456ca62246", "version": "38.00.000"}, "exchange direction": "INPUT", "meanAmount": 0.0, "other": {"anies": [{"value": "0.98", "module": "A1-A3"}, {"value": "1.47E-4", "module": "A4"}, {"value": "2.05E-5", "module": "A5"}, {"value": "0.0", "module": "B1"}, {"value": "0.0", "module": "B2"}, {"value": "0.0", "module": "B3"}, {"value": "0.0", "module": "B4"}, {"value": "0.0", "module": "B5"}, {"value": "1.35", "module": "B6"}, {"value": "0.0", "module": "B7"}, {"value": "-3.54E-5", "module": "C1"}, {"value": "1.07E-5", "module": "C2"}, {"value": "1.04E-4", "module": "C3"}, {"value": "-3.3E-4", "module": "C4"}, {"value": "-0.17", "module": "D"}, {"name": "referenceToUnitGroupDataSet", "value": {"shortDescription": [{"value": "m3"}], "type": "unit group data set", "refObjectId": "cd950537-0a98-4044-9ba7-9f9a68d0a504", "uri": "../unitgroups/cd950537-0a98-4044-9ba7-9f9a68d0a504"}}]}, "flowProperties": [], "typeOfFlow": "Other flow", "classification": {"classHierarchy": "Quantities / Environmental quantities / EPD EN 15804 / LCI indicators", "name": "GaBiCategories"}}, {"dataSetInternalID": 9, "referenceToFlowDataSet": {"shortDescription": [{"value": "Non-hazardous waste disposed (NHWD)", "lang": "en"}, {"value": "Ungefährlicher Abfall zur Beseitigung (NHWD)", "lang": "de"}], "type": "flow data set", "refObjectId": "b29ef66b-e286-4afa-949f-62f1a7b4d7fa", "version": "38.00.000"}, "exchange direction": "OUTPUT", "meanAmount": 0.0, "other": {"anies": [{"value": "359.0", "module": "A1-A3"}, {"value": "0.0317", "module": "A4"}, {"value": "0.11", "module": "A5"}, {"value": "0.0", "module": "B1"}, {"value": "0.0", "module": "B2"}, {"value": "0.0", "module": "B3"}, {"value": "0.0", "module": "B4"}, {"value": "0.0", "module": "B5"}, {"value": "306.0", "module": "B6"}, {"value": "0.0", "module": "B7"}, {"value": "0.0481", "module": "C1"}, {"value": "0.00228", "module": "C2"}, {"value": "0.0388", "module": "C3"}, {"value": "0.45", "module": "C4"}, {"value": "-105.0", "module": "D"}, {"name": "referenceToUnitGroupDataSet", "value": {"shortDescription": [{"value": "kg"}], "type": "unit group data set", "refObjectId": "ad38d542-3fe9-439d-9b95-2f5f7752acaf", "uri": "../unitgroups/ad38d542-3fe9-439d-9b95-2f5f7752acaf"}}]}, "flowProperties": [], "typeOfFlow": "Other flow", "classification": {"classHierarchy": "Quantities / Environmental quantities / EPD EN 15804 / LCI indicators", "name": "GaBiCategories"}}, {"dataSetInternalID": 10, "referenceToFlowDataSet": {"shortDescription": [{"value": "Nicht-erneuerbare Primärenergie als Energieträger (PENRE)", "lang": "en"}, {"value": "Nicht-erneuerbare Primärenergie als Energieträger (PENRE)", "lang": "de"}], "type": "flow data set", "refObjectId": "ac857178-2b45-46ec-892a-a9a4332f0372", "version": "38.00.000"}, "exchange direction": "INPUT", "meanAmount": 0.0, "other": {"anies": [{"value": "1500.0", "module": "A1-A3"}, {"value": "1.01", "module": "A4"}, {"value": "0.0256", "module": "A5"}, {"value": "0.0", "module": "B1"}, {"value": "0.0", "module": "B2"}, {"value": "0.0", "module": "B3"}, {"value": "0.0", "module": "B4"}, {"value": "0.0", "module": "B5"}, {"value": "1570.0", "module": "B6"}, {"value": "0.0", "module": "B7"}, {"value": "0.00302", "module": "C1"}, {"value": "0.0726", "module": "C2"}, {"value": "0.23", "module": "C3"}, {"value": "0.0282", "module": "C4"}, {"value": "-261.0", "module": "D"}, {"name": "referenceToUnitGroupDataSet", "value": {"shortDescription": [{"value": "MJ"}], "type": "unit group data set", "refObjectId": "93a60a57-a3c8-11da-a746-0800200c9a66", "uri": "../unitgroups/93a60a57-a3c8-11da-a746-0800200c9a66"}}]}, "flowProperties": [], "typeOfFlow": "Other flow", "classification": {"classHierarchy": "Quantities", "name": "GaBiCategories"}}, {"dataSetInternalID": 11, "referenceToFlowDataSet": {"shortDescription": [{"value": "Nicht-erneuerbare Primärenergie zur stofflichen Nutzung (PENRM)", "lang": "en"}, {"value": "Nicht-erneuerbare Primärenergie zur stofflichen Nutzung (PENRM)", "lang": "de"}], "type": "flow data set", "refObjectId": "1421caa0-679d-4bf4-b282-0eb850ccae27", "version": "38.00.000"}, "exchange direction": "INPUT", "meanAmount": 0.0, "other": {"anies": [{"value": "1500.0", "module": "A1-A3"}, {"value": "1.01", "module": "A4"}, {"value": "0.0256", "module": "A5"}, {"value": "0.0", "module": "B1"}, {"value": "0.0", "module": "B2"}, {"value": "0.0", "module": "B3"}, {"value": "0.0", "module": "B4"}, {"value": "0.0", "module": "B5"}, {"value": "1570.0", "module": "B6"}, {"value": "0.0", "module": "B7"}, {"value": "0.00302", "module": "C1"}, {"value": "0.0726", "module": "C2"}, {"value": "0.23", "module": "C3"}, {"value": "0.0282", "module": "C4"}, {"value": "-261.0", "module": "D"}, {"name": "referenceToUnitGroupDataSet", "value": {"shortDescription": [{"value": "MJ"}], "type": "unit group data set", "refObjectId": "93a60a57-a3c8-11da-a746-0800200c9a66", "uri": "../unitgroups/93a60a57-a3c8-11da-a746-0800200c9a66"}}]}, "flowProperties": [], "typeOfFlow": "Other flow", "classification": {"classHierarchy": "Quantities", "name": "GaBiCategories"}}, {"dataSetInternalID": 12, "referenceToFlowDataSet": {"shortDescription": [{"value": "Use of non renewable secondary fuels (NRSF)", "lang": "en"}, {"value": "Verbrauch nicht erneuerbarer Sekundärbrennstoffe (NRSF)", "lang": "de"}], "type": "flow data set", "refObjectId": "89def144-d39a-4287-b86f-efde453ddcb2", "version": "38.00.000"}, "exchange direction": "INPUT", "meanAmount": 0.0, "other": {"anies": [{"value": "0.0", "module": "A1-A3"}, {"value": "0.0", "module": "A4"}, {"value": "0.0", "module": "A5"}, {"value": "0.0", "module": "B1"}, {"value": "0.0", "module": "B2"}, {"value": "0.0", "module": "B3"}, {"value": "0.0", "module": "B4"}, {"value": "0.0", "module": "B5"}, {"value": "0.0", "module": "B6"}, {"value": "0.0", "module": "B7"}, {"value": "0.0", "module": "C1"}, {"value": "0.0", "module": "C2"}, {"value": "0.0", "module": "C3"}, {"value": "0.0", "module": "C4"}, {"value": "0.0", "module": "D"}, {"name": "referenceToUnitGroupDataSet", "value": {"shortDescription": [{"value": "MJ"}], "type": "unit group data set", "refObjectId": "93a60a57-a3c8-11da-a746-0800200c9a66", "uri": "../unitgroups/93a60a57-a3c8-11da-a746-0800200c9a66"}}]}, "flowProperties": [], "typeOfFlow": "Other flow", "classification": {"classHierarchy": "Quantities / Environmental quantities / EPD EN 15804 / LCI indicators", "name": "GaBiCategories"}}, {"dataSetInternalID": 13, "referenceToFlowDataSet": {"shortDescription": [{"value": "Radioactive waste disposed (RWD)", "lang": "en"}, {"value": "Entsorgter radioaktiver Abfall (RWD)", "lang": "de"}], "type": "flow data set", "refObjectId": "3449546e-52ad-4b39-b809-9fb77cea8ff6", "version": "38.00.000"}, "exchange direction": "OUTPUT", "meanAmount": 0.0, "other": {"anies": [{"value": "0.0032", "module": "A1-A3"}, {"value": "2.16E-7", "module": "A4"}, {"value": "6.01E-9", "module": "A5"}, {"value": "0.0", "module": "B1"}, {"value": "0.0", "module": "B2"}, {"value": "0.0", "module": "B3"}, {"value": "0.0", "module": "B4"}, {"value": "0.0", "module": "B5"}, {"value": "0.0111", "module": "B6"}, {"value": "0.0", "module": "B7"}, {"value": "1.83E-9", "module": "C1"}, {"value": "1.57E-8", "module": "C2"}, {"value": "4.75E-7", "module": "C3"}, {"value": "1.7E-8", "module": "C4"}, {"value": "-4.61E-4", "module": "D"}, {"name": "referenceToUnitGroupDataSet", "value": {"shortDescription": [{"value": "kg"}], "type": "unit group data set", "refObjectId": "ad38d542-3fe9-439d-9b95-2f5f7752acaf", "uri": "../unitgroups/ad38d542-3fe9-439d-9b95-2f5f7752acaf"}}]}, "flowProperties": [], "typeOfFlow": "Other flow", "classification": {"classHierarchy": "Quantities / Environmental quantities / EPD EN 15804 / LCI indicators", "name": "GaBiCategories"}}, {"dataSetInternalID": 14, "referenceToFlowDataSet": {"shortDescription": [{"value": "Erneuerbare Primärenergie als Energieträger (PERE)", "lang": "en"}, {"value": "Erneuerbare Primärenergie als Energieträger (PERE)", "lang": "de"}], "type": "flow data set", "refObjectId": "20f32be5-0398-4288-9b6d-accddd195317", "version": "38.00.000"}, "exchange direction": "INPUT", "meanAmount": 0.0, "other": {"anies": [{"value": "162.0", "module": "A1-A3"}, {"value": "0.0132", "module": "A4"}, {"value": "4.13E-4", "module": "A5"}, {"value": "0.0", "module": "B1"}, {"value": "0.0", "module": "B2"}, {"value": "0.0", "module": "B3"}, {"value": "0.0", "module": "B4"}, {"value": "0.0", "module": "B5"}, {"value": "429.0", "module": "B6"}, {"value": "0.0", "module": "B7"}, {"value": "9.36E-5", "module": "C1"}, {"value": "9.53E-4", "module": "C2"}, {"value": "0.0281", "module": "C3"}, {"value": "8.73E-4", "module": "C4"}, {"value": "-26.1", "module": "D"}, {"name": "referenceToUnitGroupDataSet", "value": {"shortDescription": [{"value": "MJ"}], "type": "unit group data set", "refObjectId": "93a60a57-a3c8-11da-a746-0800200c9a66", "uri": "../unitgroups/93a60a57-a3c8-11da-a746-0800200c9a66"}}]}, "flowProperties": [], "typeOfFlow": "Other flow", "classification": {"classHierarchy": "Quantities", "name": "GaBiCategories"}}, {"dataSetInternalID": 15, "referenceToFlowDataSet": {"shortDescription": [{"value": "Erneuerbare Primärenergie zur stofflichen Nutzung (PERM)", "lang": "en"}, {"value": "Erneuerbare Primärenergie zur stofflichen Nutzung (PERM)", "lang": "de"}], "type": "flow data set", "refObjectId": "fb3ec0de-548d-4508-aea5-00b73bf6f702", "version": "38.00.000"}, "exchange direction": "INPUT", "meanAmount": 0.0, "other": {"anies": [{"value": "162.0", "module": "A1-A3"}, {"value": "0.0132", "module": "A4"}, {"value": "4.13E-4", "module": "A5"}, {"value": "0.0", "module": "B1"}, {"value": "0.0", "module": "B2"}, {"value": "0.0", "module": "B3"}, {"value": "0.0", "module": "B4"}, {"value": "0.0", "module": "B5"}, {"value": "429.0", "module": "B6"}, {"value": "0.0", "module": "B7"}, {"value": "9.36E-5", "module": "C1"}, {"value": "9.53E-4", "module": "C2"}, {"value": "0.0281", "module": "C3"}, {"value": "8.73E-4", "module": "C4"}, {"value": "-26.1", "module": "D"}, {"name": "referenceToUnitGroupDataSet", "value": {"shortDescription": [{"value": "MJ"}], "type": "unit group data set", "refObjectId": "93a60a57-a3c8-11da-a746-0800200c9a66", "uri": "../unitgroups/93a60a57-a3c8-11da-a746-0800200c9a66"}}]}, "flowProperties": [], "typeOfFlow": "Other flow", "classification": {"classHierarchy": "Quantities", "name": "GaBiCategories"}}, {"dataSetInternalID": 16, "referenceToFlowDataSet": {"shortDescription": [{"value": "Use of renewable secondary fuels (RSF)", "lang": "en"}, {"value": "Erneuerbare Sekundärbrennstoffe (RSF)", "lang": "de"}], "type": "flow data set", "refObjectId": "64333088-a55f-4aa2-9a31-c10b07816787", "version": "38.00.000"}, "exchange direction": "INPUT", "meanAmount": 0.0, "other": {"anies": [{"value": "0.013", "module": "A1-A3"}, {"value": "5.42E-6", "module": "A4"}, {"value": "1.97E-7", "module": "A5"}, {"value": "0.0", "module": "B1"}, {"value": "0.0", "module": "B2"}, {"value": "0.0", "module": "B3"}, {"value": "0.0", "module": "B4"}, {"value": "0.0", "module": "B5"}, {"value": "0.00207", "module": "B6"}, {"value": "0.0", "module": "B7"}, {"value": "1.71E-8", "module": "C1"}, {"value": "3.93E-7", "module": "C2"}, {"value": "9.69E-6", "module": "C3"}, {"value": "1.6E-7", "module": "C4"}, {"value": "-0.00174", "module": "D"}, {"name": "referenceToUnitGroupDataSet", "value": {"shortDescription": [{"value": "MJ"}], "type": "unit group data set", "refObjectId": "93a60a57-a3c8-11da-a746-0800200c9a66", "uri": "../unitgroups/93a60a57-a3c8-11da-a746-0800200c9a66"}}]}, "flowProperties": [], "typeOfFlow": "Other flow", "classification": {"classHierarchy": "Quantities / Environmental quantities / EPD EN 15804 / LCI indicators", "name": "GaBiCategories"}}, {"dataSetInternalID": 17, "referenceToFlowDataSet": {"shortDescription": [{"value": "Input of secondary material (SM)", "lang": "en"}, {"value": "Einsatz von Sekundärstoffen (SM)", "lang": "de"}], "type": "flow data set", "refObjectId": "c6a1f35f-2d09-4f54-8dfb-97e502e1ce92", "version": "38.00.000"}, "exchange direction": "INPUT", "meanAmount": 0.0, "other": {"anies": [{"value": "0.31", "module": "A1-A3"}, {"value": "4.27E-4", "module": "A4"}, {"value": "1.45E-5", "module": "A5"}, {"value": "0.0", "module": "B1"}, {"value": "0.0", "module": "B2"}, {"value": "0.0", "module": "B3"}, {"value": "0.0", "module": "B4"}, {"value": "0.0", "module": "B5"}, {"value": "0.26", "module": "B6"}, {"value": "0.0", "module": "B7"}, {"value": "9.91E-7", "module": "C1"}, {"value": "3.08E-5", "module": "C2"}, {"value": "9.97E-5", "module": "C3"}, {"value": "9.24E-6", "module": "C4"}, {"value": "-0.15", "module": "D"}, {"name": "referenceToUnitGroupDataSet", "value": {"shortDescription": [{"value": "kg"}], "type": "unit group data set", "refObjectId": "ad38d542-3fe9-439d-9b95-2f5f7752acaf", "uri": "../unitgroups/ad38d542-3fe9-439d-9b95-2f5f7752acaf"}}]}, "flowProperties": [], "typeOfFlow": "Other flow", "classification": {"classHierarchy": "Quantities / Environmental quantities / EPD EN 15804 / LCI indicators", "name": "GaBiCategories"}}, {"dataSetInternalID": 18, "referenceToFlowDataSet": {"shortDescription": [{"value": "Total use of non-renewable primary energy resources (PENRT)", "lang": "en"}, {"value": "Total nicht erneuerbare Primärenergie (PENRT)", "lang": "de"}], "type": "flow data set", "refObjectId": "06159210-646b-4c8d-8583-da9b3b95a6c1", "version": "38.00.000"}, "exchange direction": "INPUT", "meanAmount": 0.0, "other": {"anies": [{"value": "1500.0", "module": "A1-A3"}, {"value": "1.01", "module": "A4"}, {"value": "0.0256", "module": "A5"}, {"value": "0.0", "module": "B1"}, {"value": "0.0", "module": "B2"}, {"value": "0.0", "module": "B3"}, {"value": "0.0", "module": "B4"}, {"value": "0.0", "module": "B5"}, {"value": "1570.0", "module": "B6"}, {"value": "0.0", "module": "B7"}, {"value": "0.00302", "module": "C1"}, {"value": "0.0726", "module": "C2"}, {"value": "0.23", "module": "C3"}, {"value": "0.0282", "module": "C4"}, {"value": "-261.0", "module": "D"}, {"name": "referenceToUnitGroupDataSet", "value": {"shortDescription": [{"value": "MJ"}], "type": "unit group data set", "refObjectId": "93a60a57-a3c8-11da-a746-0800200c9a66", "uri": "../unitgroups/93a60a57-a3c8-11da-a746-0800200c9a66"}}]}, "flowProperties": [], "typeOfFlow": "Other flow", "classification": {"classHierarchy": "Quantities / Environmental quantities / EPD EN 15804 / LCI indicators", "name": "GaBiCategories"}}, {"dataSetInternalID": 19, "referenceToFlowDataSet": {"shortDescription": [{"value": "Total use of renewable primary energy resources (PERT)", "lang": "en"}, {"value": "Gesamtverbrauch von erneuerbarer Primärenergie (PERT)", "lang": "de"}], "type": "flow data set", "refObjectId": "53f97275-fa8a-4cdd-9024-65936002acd0", "version": "38.00.000"}, "exchange direction": "INPUT", "meanAmount": 0.0, "other": {"anies": [{"value": "162.0", "module": "A1-A3"}, {"value": "0.0132", "module": "A4"}, {"value": "4.13E-4", "module": "A5"}, {"value": "0.0", "module": "B1"}, {"value": "0.0", "module": "B2"}, {"value": "0.0", "module": "B3"}, {"value": "0.0", "module": "B4"}, {"value": "0.0", "module": "B5"}, {"value": "429.0", "module": "B6"}, {"value": "0.0", "module": "B7"}, {"value": "9.36E-5", "module": "C1"}, {"value": "9.53E-4", "module": "C2"}, {"value": "0.0281", "module": "C3"}, {"value": "8.73E-4", "module": "C4"}, {"value": "-26.1", "module": "D"}, {"name": "referenceToUnitGroupDataSet", "value": {"shortDescription": [{"value": "MJ"}], "type": "unit group data set", "refObjectId": "93a60a57-a3c8-11da-a746-0800200c9a66", "uri": "../unitgroups/93a60a57-a3c8-11da-a746-0800200c9a66"}}]}, "flowProperties": [], "typeOfFlow": "Other flow", "classification": {"classHierarchy": "Quantities / Environmental quantities / EPD EN 15804 / LCI indicators", "name": "GaBiCategories"}}]}, "LCIAResults": {"LCIAResult": [{"referenceToLCIAMethodDataSet": {"shortDescription": [{"value": "Abiotic depletion potential - non-fossil resources (ADPE)", "lang": "en"}, {"value": "Potenzial für die Verknappung abiotischer Ressourcen – nicht fossile Ressourcen (ADPE)", "lang": "de"}], "type": "LCIA method data set", "refObjectId": "b2ad6494-c78d-11e6-9d9d-cec0c932ce01", "version": "01.00.011"}, "meanAmount": 0.0, "other": {"anies": [{"value": "1500.0", "module": "A1-A3"}, {"value": "1.01", "module": "A4"}, {"value": "0.0256", "module": "A5"}, {"value": "0.0", "module": "B1"}, {"value": "0.0", "module": "B2"}, {"value": "0.0", "module": "B3"}, {"value": "0.0", "module": "B4"}, {"value": "0.0", "module": "B5"}, {"value": "1570.0", "module": "B6"}, {"value": "0.0", "module": "B7"}, {"value": "0.00302", "module": "C1"}, {"value": "0.0726", "module": "C2"}, {"value": "0.23", "module": "C3"}, {"value": "0.0281", "module": "C4"}, {"value": "-261.0", "module": "D"}, {"name": "referenceToUnitGroupDataSet", "value": {"shortDescription": [{"value": "kg Sb-Äqv."}], "type": "unit group data set", "refObjectId": "54ccd2d9-a32a-4fc2-923d-f2c8c93e89d4", "uri": "../unitgroups/54ccd2d9-a32a-4fc2-923d-f2c8c93e89d4"}}]}}, {"referenceToLCIAMethodDataSet": {"shortDescription": [{"value": "Abiotic depletion potential - fossil resources (ADPF)", "lang": "en"}, {"value": "Potenzial für die Verknappung abiotischer Ressourcen – fossile Brennstoffe (ADPF)", "lang": "de"}], "type": "LCIA method data set", "refObjectId": "b2ad6110-c78d-11e6-9d9d-cec0c932ce01", "version": "01.00.011"}, "meanAmount": 0.0, "other": {"anies": [{"value": "0.0497", "module": "A1-A3"}, {"value": "1.95E-7", "module": "A4"}, {"value": "5.57E-9", "module": "A5"}, {"value": "0.0", "module": "B1"}, {"value": "0.0", "module": "B2"}, {"value": "0.0", "module": "B3"}, {"value": "0.0", "module": "B4"}, {"value": "0.0", "module": "B5"}, {"value": "9.08E-4", "module": "B6"}, {"value": "0.0", "module": "B7"}, {"value": "3.38E-10", "module": "C1"}, {"value": "1.4E-8", "module": "C2"}, {"value": "2.65E-7", "module": "C3"}, {"value": "3.15E-9", "module": "C4"}, {"value": "-0.00835", "module": "D"}, {"name": "referenceToUnitGroupDataSet", "value": {"shortDescription": [{"value": "MJ"}], "type": "unit group data set", "refObjectId": "93a60a57-a3c8-11da-a746-0800200c9a66", "uri": "../unitgroups/93a60a57-a3c8-11da-a746-0800200c9a66"}}]}}, {"referenceToLCIAMethodDataSet": {"shortDescription": [{"value": "Acidification potential, Accumulated Exceedance (AP)", "lang": "en"}, {"value": "Versauerungspotenzial, kumulierte Überschreitung (AP)", "lang": "de"}], "type": "LCIA method data set", "refObjectId": "b5c611c6-def3-11e6-bf01-fe55135034f3", "version": "01.03.010", "uri": "http://lca.jrc.ec.europa.eu/lcainfohub/datasets/elcd/lciamethods/f6cbd466-253f-4145-a4bb-8dae7d266e89.xml"}, "meanAmount": 0.0, "other": {"anies": [{"value": "0.79", "module": "A1-A3"}, {"value": "1.7E-4", "module": "A4"}, {"value": "8.37E-5", "module": "A5"}, {"value": "0.0", "module": "B1"}, {"value": "0.0", "module": "B2"}, {"value": "0.0", "module": "B3"}, {"value": "0.0", "module": "B4"}, {"value": "0.0", "module": "B5"}, {"value": "0.4", "module": "B6"}, {"value": "0.0", "module": "B7"}, {"value": "1.6E-6", "module": "C1"}, {"value": "2.07E-5", "module": "C2"}, {"value": "1.13E-4", "module": "C3"}, {"value": "1.5E-5", "module": "C4"}, {"value": "-0.19", "module": "D"}, {"name": "referenceToUnitGroupDataSet", "value": {"shortDescription": [{"value": "mol H+ eqv."}], "type": "unit group data set", "refObjectId": "42e089ac-92bf-4bf2-8ca1-5fc40d18f2ed", "uri": "../unitgroups/42e089ac-92bf-4bf2-8ca1-5fc40d18f2ed"}}]}}, {"referenceToLCIAMethodDataSet": {"shortDescription": [{"value": "Eutrophication potential - freshwater (EP-freshwater)", "lang": "en"}, {"value": "Eutrophierungspotenzial - Süßwasser (EP-freshwater)", "lang": "de"}], "type": "LCIA method data set", "refObjectId": "b53ec18f-7377-4ad3-86eb-cc3f4f276b2b", "version": "01.00.011", "uri": "http://lca.jrc.ec.europa.eu/lcainfohub/datasets/elcd/lciamethods/a4630d5b-df2f-48ae-b3f2-5e5257606d68.xml"}, "meanAmount": 0.0, "other": {"anies": [{"value": "0.17", "module": "A1-A3"}, {"value": "5.42E-6", "module": "A4"}, {"value": "2.86E-6", "module": "A5"}, {"value": "0.0", "module": "B1"}, {"value": "0.0", "module": "B2"}, {"value": "0.0", "module": "B3"}, {"value": "0.0", "module": "B4"}, {"value": "0.0", "module": "B5"}, {"value": "0.0626", "module": "B6"}, {"value": "0.0", "module": "B7"}, {"value": "7.14E-7", "module": "C1"}, {"value": "3.91E-7", "module": "C2"}, {"value": "7.86E-6", "module": "C3"}, {"value": "6.66E-6", "module": "C4"}, {"value": "-0.0263", "module": "D"}, {"name": "referenceToUnitGroupDataSet", "value": {"shortDescription": [{"value": "kg P eqv."}], "type": "unit group data set", "refObjectId": "0429039d-a61d-4590-ba67-aa4a20a810a1", "uri": "../unitgroups/0429039d-a61d-4590-ba67-aa4a20a810a1"}}]}}, {"referenceToLCIAMethodDataSet": {"shortDescription": [{"value": "Eutrophication potential - marine (EP-marine)", "lang": "en"}, {"value": "Eutrophierungspotenzial - Salzwasser (EP-marine)", "lang": "de"}], "type": "LCIA method data set", "refObjectId": "b5c619fa-def3-11e6-bf01-fe55135034f3", "version": "02.00.011", "uri": "http://lca.jrc.ec.europa.eu/lcainfohub/datasets/elcd/lciamethods/5296e2be-060b-4e50-b033-d45f85f6ac92.xml"}, "meanAmount": 0.0, "other": {"anies": [{"value": "0.17", "module": "A1-A3"}, {"value": "4.29E-5", "module": "A4"}, {"value": "1.95E-4", "module": "A5"}, {"value": "0.0", "module": "B1"}, {"value": "0.0", "module": "B2"}, {"value": "0.0", "module": "B3"}, {"value": "0.0", "module": "B4"}, {"value": "0.0", "module": "B5"}, {"value": "0.0621", "module": "B6"}, {"value": "0.0", "module": "B7"}, {"value": "1.34E-5", "module": "C1"}, {"value": "7.54E-6", "module": "C2"}, {"value": "2.49E-5", "module": "C3"}, {"value": "1.25E-4", "module": "C4"}, {"value": "-0.0297", "module": "D"}, {"name": "referenceToUnitGroupDataSet", "value": {"shortDescription": [{"value": "kg N eqv."}], "type": "unit group data set", "refObjectId": "d05bb823-ecdf-4686-8c40-bf1d9257859f", "uri": "../unitgroups/d05bb823-ecdf-4686-8c40-bf1d9257859f"}}]}}, {"referenceToLCIAMethodDataSet": {"shortDescription": [{"value": "Eutrophication potential - terrestrial (EP-terrestrial)", "lang": "en"}, {"value": "Eutrophierungspotenzial - Land (EP-terrestrial)", "lang": "de"}], "type": "LCIA method data set", "refObjectId": "b5c614d2-def3-11e6-bf01-fe55135034f3", "version": "01.02.010", "uri": "http://lca.jrc.ec.europa.eu/lcainfohub/datasets/elcd/lciamethods/40054970-5936-477c-9bec-29fa23b1cb77.xml"}, "meanAmount": 0.0, "other": {"anies": [{"value": "1.82", "module": "A1-A3"}, {"value": "4.65E-4", "module": "A4"}, {"value": "4.23E-4", "module": "A5"}, {"value": "0.0", "module": "B1"}, {"value": "0.0", "module": "B2"}, {"value": "0.0", "module": "B3"}, {"value": "0.0", "module": "B4"}, {"value": "0.0", "module": "B5"}, {"value": "0.56", "module": "B6"}, {"value": "0.0", "module": "B7"}, {"value": "4.99E-6", "module": "C1"}, {"value": "8.21E-5", "module": "C2"}, {"value": "2.64E-4", "module": "C3"}, {"value": "4.65E-5", "module": "C4"}, {"value": "-0.33", "module": "D"}, {"name": "referenceToUnitGroupDataSet", "value": {"shortDescription": [{"value": "mol N eqv."}], "type": "unit group data set", "refObjectId": "71b4d617-0ec9-4d3f-b65e-e438940c2401", "uri": "../unitgroups/71b4d617-0ec9-4d3f-b65e-e438940c2401"}}]}}, {"referenceToLCIAMethodDataSet": {"shortDescription": [{"value": "Global Warming Potential - total (GWP-total)", "lang": "en"}, {"value": "Globales Erwärmungspotenzial - total (GWP-total)", "lang": "de"}], "type": "LCIA method data set", "refObjectId": "6a37f984-a4b3-458a-a20a-64418c145fa2", "version": "04.00.017"}, "meanAmount": 0.0, "other": {"anies": [{"value": "115.0", "module": "A1-A3"}, {"value": "0.0671", "module": "A4"}, {"value": "0.38", "module": "A5"}, {"value": "0.0", "module": "B1"}, {"value": "0.0", "module": "B2"}, {"value": "0.0", "module": "B3"}, {"value": "0.0", "module": "B4"}, {"value": "0.0", "module": "B5"}, {"value": "69.9", "module": "B6"}, {"value": "0.0", "module": "B7"}, {"value": "0.00697", "module": "C1"}, {"value": "0.00497", "module": "C2"}, {"value": "0.0192", "module": "C3"}, {"value": "0.065", "module": "C4"}, {"value": "-18.7", "module": "D"}, {"name": "referenceToUnitGroupDataSet", "value": {"shortDescription": [{"value": "kg CO2-Äqv."}], "type": "unit group data set", "refObjectId": "1ebf3012-d0db-4de2-aefd-ef30cedb0be1", "uri": "../unitgroups/1ebf3012-d0db-4de2-aefd-ef30cedb0be1"}}]}}, {"referenceToLCIAMethodDataSet": {"shortDescription": [{"value": "Global Warming Potential - fossil fuels (GWP-fossil)", "lang": "en"}, {"value": "Globales Erwärmungspotenzial - fossil (GWP-fossil)", "lang": "de"}], "type": "LCIA method data set", "refObjectId": "5f635281-343e-44fb-83df-1971b155e6b6", "version": "01.00.009"}, "meanAmount": 0.0, "other": {"anies": [{"value": "115.0", "module": "A1-A3"}, {"value": "0.0671", "module": "A4"}, {"value": "0.0108", "module": "A5"}, {"value": "0.0", "module": "B1"}, {"value": "0.0", "module": "B2"}, {"value": "0.0", "module": "B3"}, {"value": "0.0", "module": "B4"}, {"value": "0.0", "module": "B5"}, {"value": "67.3", "module": "B6"}, {"value": "0.0", "module": "B7"}, {"value": "4.76E-4", "module": "C1"}, {"value": "0.00497", "module": "C2"}, {"value": "0.0184", "module": "C3"}, {"value": "0.00444", "module": "C4"}, {"value": "-18.7", "module": "D"}, {"name": "referenceToUnitGroupDataSet", "value": {"shortDescription": [{"value": "kg CO2-Äqv."}], "type": "unit group data set", "refObjectId": "1ebf3012-d0db-4de2-aefd-ef30cedb0be1", "uri": "../unitgroups/1ebf3012-d0db-4de2-aefd-ef30cedb0be1"}}]}}, {"referenceToLCIAMethodDataSet": {"shortDescription": [{"value": "Global Warming Potential - biogenic (GWP-biogenic)", "lang": "en"}, {"value": "Globales Erwärmungspotenzial - biogen (GWP-biogenic)", "lang": "de"}], "type": "LCIA method data set", "refObjectId": "2356e1ab-0185-4db5-86e5-16de51c7485c", "version": "01.00.006"}, "meanAmount": 0.0, "other": {"anies": [{"value": "0.23", "module": "A1-A3"}, {"value": "2.63E-6", "module": "A4"}, {"value": "0.36", "module": "A5"}, {"value": "0.0", "module": "B1"}, {"value": "0.0", "module": "B2"}, {"value": "0.0", "module": "B3"}, {"value": "0.0", "module": "B4"}, {"value": "0.0", "module": "B5"}, {"value": "2.37", "module": "B6"}, {"value": "0.0", "module": "B7"}, {"value": "0.0065", "module": "C1"}, {"value": "1.59E-7", "module": "C2"}, {"value": "8.52E-4", "module": "C3"}, {"value": "0.0606", "module": "C4"}, {"value": "1.36E-4", "module": "D"}, {"name": "referenceToUnitGroupDataSet", "value": {"shortDescription": [{"value": "kg CO2-Äqv."}], "type": "unit group data set", "refObjectId": "1ebf3012-d0db-4de2-aefd-ef30cedb0be1", "uri": "../unitgroups/1ebf3012-d0db-4de2-aefd-ef30cedb0be1"}}]}}, {"referenceToLCIAMethodDataSet": {"shortDescription": [{"value": "Global Warming Potential - land use and land use change (GWP-luluc)", "lang": "en"}, {"value": "Globales Erwärmungspotenzial - luluc (GWP-luluc)", "lang": "de"}], "type": "LCIA method data set", "refObjectId": "4331bbdb-978a-490d-8707-eeb047f01a55", "version": "01.00.006"}, "meanAmount": 0.0, "other": {"anies": [{"value": "0.15", "module": "A1-A3"}, {"value": "2.79E-5", "module": "A4"}, {"value": "6.77E-7", "module": "A5"}, {"value": "0.0", "module": "B1"}, {"value": "0.0", "module": "B2"}, {"value": "0.0", "module": "B3"}, {"value": "0.0", "module": "B4"}, {"value": "0.0", "module": "B5"}, {"value": "0.21", "module": "B6"}, {"value": "0.0", "module": "B7"}, {"value": "1.34E-7", "module": "C1"}, {"value": "2.02E-6", "module": "C2"}, {"value": "2.7E-5", "module": "C3"}, {"value": "1.25E-6", "module": "C4"}, {"value": "-0.0228", "module": "D"}, {"name": "referenceToUnitGroupDataSet", "value": {"shortDescription": [{"value": "kg CO2-Äqv."}], "type": "unit group data set", "refObjectId": "1ebf3012-d0db-4de2-aefd-ef30cedb0be1", "uri": "../unitgroups/1ebf3012-d0db-4de2-aefd-ef30cedb0be1"}}]}}, {"referenceToLCIAMethodDataSet": {"shortDescription": [{"value": "Depletion potential of the stratospheric ozone layer (ODP)", "lang": "en"}, {"value": "Abbaupotenzial der stratosphärischen Ozonschicht (ODP)", "lang": "de"}], "type": "LCIA method data set", "refObjectId": "b5c629d6-def3-11e6-bf01-fe55135034f3", "version": "02.00.013", "uri": "http://lca.jrc.ec.europa.eu/lcainfohub/datasets/elcd/lciamethods/8b723200-3d8f-4eec-9e10-444edb029476.xml"}, "meanAmount": 0.0, "other": {"anies": [{"value": "6.31E-6", "module": "A1-A3"}, {"value": "1.07E-9", "module": "A4"}, {"value": "2.97E-11", "module": "A5"}, {"value": "0.0", "module": "B1"}, {"value": "0.0", "module": "B2"}, {"value": "0.0", "module": "B3"}, {"value": "0.0", "module": "B4"}, {"value": "0.0", "module": "B5"}, {"value": "1.24E-6", "module": "B6"}, {"value": "0.0", "module": "B7"}, {"value": "3.2E-12", "module": "C1"}, {"value": "7.75E-11", "module": "C2"}, {"value": "1.5E-10", "module": "C3"}, {"value": "2.98E-11", "module": "C4"}, {"value": "-4.85E-7", "module": "D"}, {"name": "referenceToUnitGroupDataSet", "value": {"shortDescription": [{"value": "kg CFC 11-Äquiv."}], "type": "unit group data set", "refObjectId": "d9e957c9-7309-4474-bf3a-7777df6c4e5b", "uri": "../unitgroups/d9e957c9-7309-4474-bf3a-7777df6c4e5b"}}]}}, {"referenceToLCIAMethodDataSet": {"shortDescription": [{"value": "Photochemical Ozone Creation Potential (POCP)", "lang": "en"}, {"value": "Bildungspotenzial für troposphärisches Ozon (POCP)", "lang": "de"}], "type": "LCIA method data set", "refObjectId": "b5c610fe-def3-11e6-bf01-fe55135034f3", "version": "02.00.015", "uri": "http://lca.jrc.ec.europa.eu/lcainfohub/datasets/elcd/lciamethods/ec7836be-83eb-41da-bcda-1a6a3fe2d149.xml"}, "meanAmount": 0.0, "other": {"anies": [{"value": "0.52", "module": "A1-A3"}, {"value": "2.56E-4", "module": "A4"}, {"value": "2.19E-4", "module": "A5"}, {"value": "3.1E-6", "module": "B1"}, {"value": "0.0", "module": "B2"}, {"value": "0.0", "module": "B3"}, {"value": "0.0", "module": "B4"}, {"value": "0.0", "module": "B5"}, {"value": "0.18", "module": "B6"}, {"value": "0.0", "module": "B7"}, {"value": "3.15E-6", "module": "C1"}, {"value": "3.01E-5", "module": "C2"}, {"value": "7.76E-5", "module": "C3"}, {"value": "2.94E-5", "module": "C4"}, {"value": "-0.13", "module": "D"}, {"name": "referenceToUnitGroupDataSet", "value": {"shortDescription": [{"value": "kg NMVOC eqv."}], "type": "unit group data set", "refObjectId": "d27c25f8-fbc1-44c6-b47b-4adbae4199c6", "uri": "../unitgroups/d27c25f8-fbc1-44c6-b47b-4adbae4199c6"}}]}}, {"referenceToLCIAMethodDataSet": {"shortDescription": [{"value": "Water (user) deprivation potential (WDP)", "lang": "en"}, {"value": "Wasser-Entzugspotenzial (Benutzer) (WDP)", "lang": "de"}], "type": "LCIA method data set", "refObjectId": "b2ad66ce-c78d-11e6-9d9d-cec0c932ce01", "version": "03.00.015"}, "meanAmount": 0.0, "other": {"anies": [{"value": "36.9", "module": "A1-A3"}, {"value": "0.0048", "module": "A4"}, {"value": "0.00158", "module": "A5"}, {"value": "0.0", "module": "B1"}, {"value": "0.0", "module": "B2"}, {"value": "0.0", "module": "B3"}, {"value": "0.0", "module": "B4"}, {"value": "0.0", "module": "B5"}, {"value": "42.6", "module": "B6"}, {"value": "0.0", "module": "B7"}, {"value": "3.18E-5", "module": "C1"}, {"value": "3.48E-4", "module": "C2"}, {"value": "0.00363", "module": "C3"}, {"value": "2.97E-4", "module": "C4"}, {"value": "-6.01", "module": "D"}, {"name": "referenceToUnitGroupDataSet", "value": {"shortDescription": [{"value": "m3 world eqv."}], "type": "unit group data set", "refObjectId": "6ae2df01-888e-46c8-b17d-49fa3869b476", "uri": "../unitgroups/6ae2df01-888e-46c8-b17d-49fa3869b476"}}]}}, {"referenceToLCIAMethodDataSet": {"shortDescription": [{"value": "Potential incidence of disease due to PM emissions (PM)", "lang": "en"}, {"value": "Potenzielles Auftreten von Krankheiten aufgrund von Feinstaubemissionen (PM)", "lang": "de"}], "type": "LCIA method data set", "refObjectId": "b5c602c6-def3-11e6-bf01-fe55135034f3", "version": "02.00.012", "uri": "http://lca.jrc.ec.europa.eu/lcainfohub/datasets/elcd/lciamethods/72ce3013-f678-4c6a-935b-f4752ff8901b.xml"}, "meanAmount": 0.0, "other": {"anies": [{"value": "6.49E-6", "module": "A1-A3"}, {"value": "6.47E-9", "module": "A4"}, {"value": "2.14E-8", "module": "A5"}, {"value": "0.0", "module": "B1"}, {"value": "0.0", "module": "B2"}, {"value": "0.0", "module": "B3"}, {"value": "0.0", "module": "B4"}, {"value": "0.0", "module": "B5"}, {"value": "1.41E-6", "module": "B6"}, {"value": "0.0", "module": "B7"}, {"value": "2.16E-11", "module": "C1"}, {"value": "5.09E-10", "module": "C2"}, {"value": "1.53E-9", "module": "C3"}, {"value": "2.01E-10", "module": "C4"}, {"value": "-1.22E-6", "module": "D"}, {"name": "referenceToUnitGroupDataSet", "value": {"shortDescription": [{"value": "disease incidence"}], "type": "unit group data set", "refObjectId": "3883559b-648f-4afc-8ba2-0bd24f3affa3", "uri": "../unitgroups/3883559b-648f-4afc-8ba2-0bd24f3affa3"}}]}}, {"referenceToLCIAMethodDataSet": {"shortDescription": [{"value": "Potential Human exposure efficiency relative to U235 (IRP)", "lang": "en"}, {"value": "Potenzielle Wirkung durch Exposition des Menschen mit U235 (IRP)", "lang": "de"}], "type": "LCIA method data set", "refObjectId": "b5c632be-def3-11e6-bf01-fe55135034f3", "version": "01.00.012", "uri": "http://lca.jrc.ec.europa.eu/lcainfohub/datasets/elcd/lciamethods/a6f4cbc8-5388-44d6-9a67-53d05684f93e.xml"}, "meanAmount": 0.0, "other": {"anies": [{"value": "13.0", "module": "A1-A3"}, {"value": "8.84E-4", "module": "A4"}, {"value": "2.43E-5", "module": "A5"}, {"value": "0.0", "module": "B1"}, {"value": "0.0", "module": "B2"}, {"value": "0.0", "module": "B3"}, {"value": "0.0", "module": "B4"}, {"value": "0.0", "module": "B5"}, {"value": "43.2", "module": "B6"}, {"value": "0.0", "module": "B7"}, {"value": "7.47E-6", "module": "C1"}, {"value": "6.41E-5", "module": "C2"}, {"value": "0.00194", "module": "C3"}, {"value": "6.97E-5", "module": "C4"}, {"value": "-1.87", "module": "D"}, {"name": "referenceToUnitGroupDataSet", "value": {"shortDescription": [{"value": "kBq U235 eqv."}], "type": "unit group data set", "refObjectId": "456b05bf-1415-44a9-9993-02452f554c09", "uri": "../unitgroups/456b05bf-1415-44a9-9993-02452f554c09"}}]}}, {"referenceToLCIAMethodDataSet": {"shortDescription": [{"value": "Potential Comparative Toxic Unit for ecosystems (ETP-fw)", "lang": "en"}, {"value": "Potenzielle Toxizitätsvergleichseinheit für Ökosysteme (ETP-fw)", "lang": "de"}], "type": "LCIA method data set", "refObjectId": "ee1082d1-b0f7-43ca-a1f0-21e2a4a74511", "version": "01.00.003", "uri": "http://lca.jrc.ec.europa.eu/lcainfohub/datasets/elcd/lciamethods/ee1082d1-b0f7-43ca-a1f0-21e2a4a74511.xml"}, "meanAmount": 0.0, "other": {"anies": [{"value": "3730.0", "module": "A1-A3"}, {"value": "0.24", "module": "A4"}, {"value": "0.92", "module": "A5"}, {"value": "2.53E-5", "module": "B1"}, {"value": "0.0", "module": "B2"}, {"value": "0.0", "module": "B3"}, {"value": "0.0", "module": "B4"}, {"value": "0.0", "module": "B5"}, {"value": "280.0", "module": "B6"}, {"value": "0.0", "module": "B7"}, {"value": "0.0938", "module": "C1"}, {"value": "0.0175", "module": "C2"}, {"value": "0.1", "module": "C3"}, {"value": "0.88", "module": "C4"}, {"value": "-634.0", "module": "D"}, {"name": "referenceToUnitGroupDataSet", "value": {"shortDescription": [{"value": "CTUe"}], "type": "unit group data set", "refObjectId": "aa959ded-f1eb-4efb-9c5c-2d60be36b3e6", "uri": "../unitgroups/aa959ded-f1eb-4efb-9c5c-2d60be36b3e6"}}]}}, {"referenceToLCIAMethodDataSet": {"shortDescription": [{"value": "Potential Comparative Toxic Unit for humans - cancer effects (HTP-c)", "lang": "en"}, {"value": "Potenzielle Toxizitätsvergleichseinheit für den Menschen - kanzerogene Wirkung (HTP-c)", "lang": "de"}], "type": "LCIA method data set", "refObjectId": "2299222a-bbd8-474f-9d4f-4dd1f18aea7c", "version": "01.00.004", "uri": "http://lca.jrc.ec.europa.eu/lcainfohub/datasets/elcd/lciamethods/2299222a-bbd8-474f-9d4f-4dd1f18aea7c.xml"}, "meanAmount": 0.0, "other": {"anies": [{"value": "2.82E-7", "module": "A1-A3"}, {"value": "3.43E-10", "module": "A4"}, {"value": "2.96E-10", "module": "A5"}, {"value": "0.0", "module": "B1"}, {"value": "0.0", "module": "B2"}, {"value": "0.0", "module": "B3"}, {"value": "0.0", "module": "B4"}, {"value": "0.0", "module": "B5"}, {"value": "1.6E-7", "module": "B6"}, {"value": "0.0", "module": "B7"}, {"value": "9.74E-13", "module": "C1"}, {"value": "2.49E-11", "module": "C2"}, {"value": "6.93E-11", "module": "C3"}, {"value": "9.08E-12", "module": "C4"}, {"value": "-7.03E-8", "module": "D"}, {"name": "referenceToUnitGroupDataSet", "value": {"shortDescription": [{"value": "CTUh"}], "type": "unit group data set", "refObjectId": "d4c9523e-2d7e-49fd-8469-998f547d3a70", "uri": "../unitgroups/d4c9523e-2d7e-49fd-8469-998f547d3a70"}}]}}, {"referenceToLCIAMethodDataSet": {"shortDescription": [{"value": "Potential Comparative Toxic Unit for humans - non-cancer effects (HTP-nc)", "lang": "en"}, {"value": "Potenzielle Toxizitätsvergleichseinheit für den Menschen - nicht kanzerogene Wirkung (HTP-nc)", "lang": "de"}], "type": "LCIA method data set", "refObjectId": "3af763a5-b7a1-48c9-9cee-1f223481fcef", "version": "01.00.003", "uri": "http://lca.jrc.ec.europa.eu/lcainfohub/datasets/elcd/lciamethods/3af763a5-b7a1-48c9-9cee-1f223481fcef.xml"}, "meanAmount": 0.0, "other": {"anies": [{"value": "4.06E-6", "module": "A1-A3"}, {"value": "6.58E-10", "module": "A4"}, {"value": "2.87E-8", "module": "A5"}, {"value": "6.73E-13", "module": "B1"}, {"value": "0.0", "module": "B2"}, {"value": "0.0", "module": "B3"}, {"value": "0.0", "module": "B4"}, {"value": "0.0", "module": "B5"}, {"value": "1.18E-6", "module": "B6"}, {"value": "0.0", "module": "B7"}, {"value": "4.46E-11", "module": "C1"}, {"value": "4.8E-11", "module": "C2"}, {"value": "5.71E-10", "module": "C3"}, {"value": "4.16E-10", "module": "C4"}, {"value": "-6.85E-7", "module": "D"}, {"name": "referenceToUnitGroupDataSet", "value": {"shortDescription": [{"value": "CTUh"}], "type": "unit group data set", "refObjectId": "d4c9523e-2d7e-49fd-8469-998f547d3a70", "uri": "../unitgroups/d4c9523e-2d7e-49fd-8469-998f547d3a70"}}]}}, {"referenceToLCIAMethodDataSet": {"shortDescription": [{"value": "Potential Soil quality index (SQP)", "lang": "en"}, {"value": "Potenzieller Bodenqualitätsindex (SQP)", "lang": "de"}], "type": "LCIA method data set", "refObjectId": "b2ad6890-c78d-11e6-9d9d-cec0c932ce01", "version": "01.00.011"}, "meanAmount": 0.0, "other": {"anies": [{"value": "580.0", "module": "A1-A3"}, {"value": "0.99", "module": "A4"}, {"value": "0.0707", "module": "A5"}, {"value": "0.0", "module": "B1"}, {"value": "0.0", "module": "B2"}, {"value": "0.0", "module": "B3"}, {"value": "0.0", "module": "B4"}, {"value": "0.0", "module": "B5"}, {"value": "348.0", "module": "B6"}, {"value": "0.0", "module": "B7"}, {"value": "0.00563", "module": "C1"}, {"value": "0.0731", "module": "C2"}, {"value": "0.14", "module": "C3"}, {"value": "0.0525", "module": "C4"}, {"value": "-143.0", "module": "D"}, {"name": "referenceToUnitGroupDataSet", "value": {"shortDescription": [{"value": "dimensionless"}], "type": "unit group data set", "refObjectId": "f130951c-e67f-4f7f-8dd4-665de3974e18", "uri": "../unitgroups/f130951c-e67f-4f7f-8dd4-665de3974e18"}}]}}]}, "otherAttributes": {"{http://www.indata.network/EPD/2019}epd-version": "1.2", "{http://www.okworx.com/ILCD/Extensions/2018/Profile}profile": "EN_15804_A2"}, "version": "1.1"}