{"processInformation": {"dataSetInformation": {"UUID": "f721d148-f727-4a55-b2e6-52ecb90e09be", "name": {"baseName": [{"value": "Mineralwolle-Dämmstoff im niedrigen Rohdichtebereich", "lang": "de"}, {"value": "Mineral wool insulation (low bulk density range)", "lang": "en"}], "functionalUnitFlowProperties": [{"lang": "de"}]}, "classificationInformation": {"classification": [{"class": [{"value": "Dämmstoffe", "level": 0, "classId": "2"}, {"value": "Mineralwolle", "level": 1, "classId": "2.1"}, {"value": "Mineralwolle", "level": 2, "classId": "2.1.01"}], "name": "OEKOBAU.DAT"}, {"class": [{"value": "02 Bauprodukte", "level": 0}, {"value": "Wärmedämmungsprodukte", "level": 1}, {"value": "Mineralische Dämmstoffe", "level": 2}], "name": "IBUCategories"}]}, "generalComment": [{"value": "Mineralwolle ist der Oberbegriff fr Dmmstoffe aus Glas- und Steinwolle. Diese sind nichtbrennbare Dmmstoffe, welche hauptschlich aus amorphen Fasern bestehen, die aus einer silikatischen Schmelze gewonnen werden.\n\nDie in dieser Deklaration beschriebenen Mineralwolle-Dmmstoffe werden in Form von Rollen, Platten, Matten, Lamellenmatten sowie loser Wolle (Stopfwolle) und Einblaswolle im niedrigen Rohdichtebereich (bis 60 kg/m) hergestellt. Die konfektionierten Produkte werden in Dicken zwischen 10 mm und 400 mm geliefert.\n\nFr bestimmte Anwendungsbereiche werden die Dmmstoffe ein- oder zweiseitig mit einer Funktionskaschierung versehen. DieUmweltwirkungen der Kaschierungen werden im Anhang auf Basis von 1 m dargestellt.", "lang": "de"}, {"value": "Mineral wool is the generic term for insulating materials made of glass wool and stone wool. These are non-combustible insulating materials, which consist mainly of amorphous fibres obtained from a silicate melt.\n\nThe mineral wool insulation materials described in this declaration are produced in the form of rolls, boards, mats, lamella mats as well as loose-fill insulation and blowing wool in the low bulk density range (up to 60 kg/m). The ready-made products are supplied in thicknesses between 10 mm and \n400 mm.\n\nFor certain applications, the insulation materials are provided with a functional facing on one or both sides. The environmental effects of the facings are shown in the appendix on the basis of 1 m.", "lang": "en"}]}, "quantitativeReference": {"referenceToReferenceFlow": [0]}, "time": {"referenceYear": 2023, "dataSetValidUntil": 2028, "other": {"anies": [{"name": "publicationDateOfEPD", "value": 1687996800000}]}}, "geography": {"locationOfOperationSupplyOrProduction": {"location": "DE"}}, "technology": {"technologyDescriptionAndIncludedProcesses": [{"value": "Zur Herstellung werden zunächst die erforderlichen Mengen an Rohmaterial abgewogen, gemischt und einem Schmelzofen zugeführt. Das Ausgangsmaterial wird in einem Ofen bei Temperaturen von ca. 1.400-1.500 °C geschmolzen. Die Herstellung der Fasern ist produktabhängig. Zum Einsatz kommen drei Verfahren: - Zieh-Blas-Verfahren (v. a. Glaswolle): Nach dem Durchlaufen des Schmelzofens wird die glasartige Schmelze zerfasert, indem ein dünner Glasstrahl in einen sich schnell drehenden Metallkorb trifft und dort durch tausende kleine Löcher, die sich in der Außenwand des Korbes befinden, herausgeschleudert wird. Die dabei entstehenden Fäden werden mittels Gasbrenner und Druckluft zu Fasern ausgezogen. - Schleuderverfahren (Steinwolle): Nach dem Durchlaufen des Kupolofens tritt ein Strahl der flüssigen Schmelze auf sich schnell drehende Metallwalzen und wird durch die Drehbewegung zu Fasern geschleudert. - Düsenblasverfahren (Steinwolle): Nach dem Durchlaufen des Schmelzofens fließt die Glasschmelze durch eine Vielzahl von Düsen. Die dabei entstehenden Fäden werden durch Druckluft oder hochgespannten Dampf zu Fasern ausgezogen. Zur Gewährleistung der Formstabilität sowie zur Staubminderung und Hydrophobierung werden die Fasern mit einer wässrigen Lösung aus Bindemittel, Staubbindeöl, Haftvermittler und – produktabhängig – Silikonen besprüht und anschließend auf unter Unterdruck stehenden Transportbändern abgelegt. Optional können anschließend Kaschierungen aufgebracht werden (die entsprechenden Umweltwirkungen hierzu werden im Anhang angegeben). In einem kontinuierlich laufenden Härteofen erfolgt das Aushärten des Bindemittels bei oberhalb 200 °C. Struktur und Dichte des Produkts können hierbei an die genauen Einsatzanforderungen angepasst werden. Die Mineralwolle wird entsprechend der gewünschten Größe und Form zurechtgeschnitten bzw. abgelängt, zum Beispiel in Form von Rollen, Matten oder Platten. Die fertigen Produkte werden verpackt und für den Versand vorbereitet. Abschnitte und andere Reste aus Mineralwolle werden wieder in den Produktionsprozess zurückgeführt. Gütesicherung: - RAL-GZ 388 - Eigen- und Fremdüberwachung gem. CE-Kennzeichnung nach europäischen Vorschriften - KEYMARK gem. Insulation KEYMARK Scheme Rules 2.1; für Produkte der technischen Isolierung nach VDI 2055 entsprechend KEYMARK Scheme Rules und AGI-Q 132 - EUCEB - Qualitätsmanagementsystem gemäß DIN EN ISO 9001 - Für technische Isolierung produktabhängig durch VDI 2055 / AGI-Q 132 \nDeklarierte Einheit: \nDie vorliegende Umwelt-Produktdeklaration bezieht sich auf eine deklarierte Einheit von 1 m unkaschiertem bzw. unbeschichtetem Mineralwolle-Dmmstoff mit einer deklarierten Rohdichte von 24 kg/m (Rohdichtebereich < 60 kg/m).", "lang": "de"}, {"value": "For production, the required quantities of the raw materials are weighed, mixed and fed into a melting furnace. The raw materials are melted in a furnace at temperatures of approx. 1,400-1,500 °C. The manufacture of the fibres depends on the product. Three processes are used: - Rotary process (mainly glass wool): After passing the melting furnace, a thin jet of glass is led into a rapidly rotating metal basket where it is ejected through thousands of small holes in the outer wall of the basket. The resulting filaments are drawn out into fibres using a gas burner and compressed air. - Cascade centrifugal process (stone wool): After passing the cupola furnace, a thin jet of the liquid melt is directed onto rapidly rotating metal wheels. Their rotational movement spins the melt into fibres. - Steam-Blown process (stone wool): After passing the melting furnace, the glass melt flows through many nozzles. The resulting filaments are drawn out into fibres by compressed air or high-pressure steam. To ensure dimensional stability and to reduce dust and make the fibres water-repellent, they are sprayed with an aqueous solution of binder, dust-binding oil, adhesive agent and - depending on the product - silicones. They are then placed on conveyor belts under negative pressure. Facings can then be applied optionally. (The corresponding environmental impacts for this are specified in the Appendix.) In a curing oven, which runs continuously, the binder is cured at above 200 °C. The structure and density of the product are adapted to the exact application requirements. The mineral wool is cut according to the desired size and shape, for example in the form of rolls, mats or boards. The finished products are packed and prepared for shipping. Cut-offs and other mineral wool residues are returned to the production process. Quality assurance: - RAL-GZ 388 - Factory production control and third-party monitoring in accordance with CE marking according to European regulations - KEYMARK according to Insulation KEYMARK Scheme Rules 2.1; for technical insulation according to VDI 2055 according to KEYMARK Scheme Rules and AGI-Q 132 - EUCEB - Quality management system according to DIN EN ISO 9001 - For technical insulation, VDI 2055 / AGI-Q 132 (depending on product) \nDeclared unit: \nThis EPD refers to a declared unit of 1 m unfaced mineral wool insulation material with a declared bulk density of 24 kg/m (low bulk density range up to 60 kg/m).", "lang": "en"}], "technologicalApplicability": [{"value": "Mineralwolle-Dmmstoffe werden sowohl in Gebuden als auch in Industrieanlagen zum Wrme-, Schall- und Brandschutz verwendet. Die Haupt-Anwendungsbereiche der in dieser EPD deklarierten Produkte sind:\n\n- Alle Anwendungsbereiche nach DIN 4108-10 fr die Anwendungsgebiete Wand, Decke und Dach mit den dort festgelegten Anforderungen hinsichtlich des Wrme- und Schallschutzes und der mechanischen Eigenschaften\n- Einblas- und Schttdmmung\n- Technische Isolierung und Haustechnik (z. B. Dmmung von Lftungs-, Heizungs- und Warmwasserrohren, Fernwrmeleitungen, Kesseln und Apparaturen)\n- Brandschutzelemente und Industrieanwendungen (z. B. Klimakanle, Feuerschutztren, Fertighauselemente, Schornsteinsysteme, Kabelabschottungen)", "lang": "de"}, {"value": "Mineral wool insulation materials are used in buildings and industrial plants for thermal insulation as well as noise and fire protection. The main application areas of the products declared in this EPD are:\n\n- All areas of application according to DIN 4108-10 for wall, ceiling and roof applications with the specified requirements regarding thermal and sound insulation and the mechanical properties\n- Blowing wool and loose-fill insulation\n- Technical insulation and building services (e.g. insulation of pipes for ventilation, heating and hot water, district heating pipelines, boilers and equipment)\n- Fire protection elements and industrial applications (e.g. air-conditioning ducts, fire protection doors, prefabricated components, chimney systems, cable penetration sealing)", "lang": "en"}]}}, "modellingAndValidation": {"LCIMethodAndAllocation": {"typeOfDataSet": "EPD", "referenceToLCAMethodDetails": [{"shortDescription": [{"value": "Mineralische Dämmstoffe.pdf", "lang": "de"}], "type": "source data set", "refObjectId": "6cf1cbdb-9439-4117-863e-032f5f5af237"}], "other": {"anies": [{"name": "subType", "value": "average dataset"}]}}, "dataSourcesTreatmentAndRepresentativeness": {"referenceToDataSource": [{"shortDescription": [{"value": "GaBi Database (all versions)", "lang": "de"}], "type": "source data set", "refObjectId": "28d74cc0-db8b-4d7e-bc44-5f6d56ce0c4a"}, {"shortDescription": [{"value": "GaBi Database Edition 2020, CUP 2020.02", "lang": "de"}], "type": "source data set", "refObjectId": "4b368ada-d799-4afc-9d41-f371f2b23781"}], "useAdviceForDataSet": [{"value": "Gültigkeitsbereich: \nBei der vorliegenden Umwelt-Produktdeklaration handelt es sich um eine Verbands-EPD. Die in der EPD dargestellte kobilanz bezieht sich auf den Lebenszyklus von 1 m Mineralwolle im niedrigen Rohdichtebereich (≤ 60 kg/m) folgender Mitglieder des Fachverband Mineralwolleindustrie e.V. (FMI):\n\n- DEUTSCHE ROCKWOOL GmbH & Co. KG: Werke Flechtingen, Gladbeck und Neuburg\n- Knauf Insulation GmbH: Werke Bernburg und St. Egidien\n- SAINT-GOBAIN ISOVER G+H AG: Werke Bergisch Gladbach, Ladenburg, Lbz und Speyer\n- URSA Deutschland GmbH: Werk Delitzsch\n\nDie verwendeten Daten decken 100 % der jhrlichen Produktion der FMI-Mitglieder in Deutschland ab.\nDiese EPD beruht berwiegend auf Produktionsdaten fr das Bezugsjahr 2019, die in den Werken erhoben und nach massebasierter Produktionsmenge gewichtet wurden. Infolge der Durchschnittsbildung ergibt sich eine mittlere Rohdichte von 24 kg/m fr Mineralwolle-Dmmstoffe im niedrigen Rohdichtebereich. \nSystemgrenze: \nDie kobilanz der Mineralwolle-Dmmstoffe beinhaltet eine cradle-to-gate (Wiege bis zum Werkstor) -Betrachtung mit den Modulen C1-C3 und Modul D (A1–A3, +C, +D). Die folgenden Lebenszyklusphasen werden in der Analyse bercksichtigt:\n\nModul A1–A3 | Produktionsstadium\nDas Produktionsstadium beinhaltet die Aufwendungen der Rohstoffversorgung (Basalt, Dolomit, Sand, Sekundrrohstoffe, Bindemittel, etc.) sowie der damit verbundenen Transporte bezogen auf die Produktionsstandorte der FMI-Mitglieder. Die Systemgrenze fr in der Produktion verwendete Sekundrrohstoffe wird nach Erreichen des Endes der Abfalleigenschaft gesetzt. Hier gilt die nach EN 15804 definierte Systemgrenze fr Sekundrrohstoffe.\nInnerhalb der Werksgrenzen werden die Prozessschritte der Verflssigung, Zerfaserung, Zufhrung des Bindemittels, Verdichten, Hrten, der Zuschnitt und die Verpackung der Mineralwolle betrachtet. Der Herstellprozess wird dazu basierend auf den Primrdaten aller betrachteten Standorte abgebildet.\n\nDie Produktion der Kaschierung fr kaschierte Produkte wird in drei separaten Anhngen zur EPD deklariert. \n\nModul A4 | Transport zur Baustelle\nDer Transport von den betrachteten Werken zum Kunden wird basierend auf einem reprsentativen Szenario als gewichteter Durchschnitt abgebildet (360 km LKW-Transport).\n\nModul A5 | Einbau ins Gebude\nFr den Einbau ins Gebude wird ein Szenario von 2 % Verschnitt gem EURIMA (2019) deklariert. Die Verluste beim Einbau in das Gebude sind stark von der Gebudegeometrie und dem spezifischen Anwendungsfall abhngig. Somit kann der Verschnittanteil im Gebudekontext stark variieren und ist auf Gebudeebene gem der tatschlichen Gegebenheiten entsprechend anzupassen.\nNeben den Verlusten beim Einbau in das Gebude beinhaltet Modul A5 die Umweltlasten aus der Verwertung der Verpackung der Produkte.\n\nModul C1 | Rckbau / Abriss\nFr die Mineralwolle-Produkte wurde ein manueller Ausbau angenommen. Die damit verbundenen Aufwnde sind vernachlssigbar, wodurch keine Umweltwirkungen aus dem Rckbau der Produkte deklariert werden.\n\nModul C2 | Transport zur Abfallbehandlung\nModul C2 beinhaltet den Transport zur Abfallbehandlung. Dazu wird der Transport via LKW ber 50 km Transportdistanz angesetzt. Dies entspricht den Empfehlungen gem EURIMA (2019).\n\nModul C3 | Abfallbehandlung\nDas angesetzte Szenario deklariert die Deponierung der Mineralwolle, wodurch keine Umweltauswirkungen aus der Abfallbehandlung der Produkte in C3 zu deklarieren sind. \n\nModul C4 | Beseitigung\nDas Modul C4 beinhaltet die durch die Deponierung der Dmmstoffe entstehenden Umweltwirkungen. Der biogene Kohlenstoff im Bindemittel der Produkte wird als Emissionen von biogenem CO2 aus der Technosphre in die natrliche Umwelt behandelt.\n\n\nModul D | Gutschriften und Lasten auerhalb der Systemgrenzen\nIn Modul D werden die Substitutionspotenziale aus der energetischen Verwertung der Verpackung deklariert.", "lang": "de"}, {"value": "Scope: \nThis Environmental Product Declaration is a generic EPD of the FMI association. The life cycle assessment presented in the EPD refers to the life cycle of 1 m mineral wool in the low bulk density range (≤ 60 kg/m) of the following members of the Fachverband Mineralwolleindustrie\ne.V. (FMI):\n\n- DEUTSCHE ROCKWOOL GmbH & Co. KG: Flechtingen, Gladbeck and Neuburg plants\n- Knauf Insulation GmbH: Bernburg and St. Egidien plants\n- SAINT-GOBAIN ISOVER G+H AG: Bergisch Gladbach, Ladenburg, Lbz and Speyer plants\n- URSA Deutschland GmbH: Delitzsch plant\n\nThe data used cover 100 % of the annual production of the FMI members in Germany.\nThis EPD is mainly based on production data for the reference year 2019, collected in the plants and weighted by mass-based production volume. As a result of averaging, an average bulk density of 24 kg/m is obtained for mineral wool insulation materials in the low bulk density range. \nSystem boundary: \nThe life cycle assessment of mineral wool insulation material includes a cradle-to-gate analysis of the products environmental impacts with options. Subsequent life cycle phases are part of the analysis:\n\nModule A1–A3 | Production stage\nThe production stage includes the upstream burdens of raw material supply (basalt, dolomite, sand, secondary raw materials, binding agents, etc.), the respective transports and the manufacturing plants of the members of the FMI. The system boundary for secondary raw materials used in production is set after the end of waste status has been reached. The system boundary for secondary raw materials is defined according to EN 15804. During production, melting in the melting furnace, fiberization, injection of binder, compacting, curing, cutting and packaging of the mineral wool are considered.\nThe manufacturing process is modelled based on the primary data of all sites considered.\n\nThe production of the facings of mineral wool products is declared in three separate appendices to the EPD. \n\nModule A4 | Transport to construction site\nThe transport from the plants to the customer is considered as a weighted average based on a representative scenario (360 km truck transport). \n\nModule A5 | Assembly\nFor installation in the building, a scenario of 2 % waste is declared according to EURIMA (2019). The losses during installation are highly dependent on the building geometry and the specific application. Thus, the percentage of waste can vary greatly in the building context and must be adjusted at the building level according to the actual conditions. In addition to the losses during installation, module A5 includes the environmental impacts from the utilization of the packaging of the products.\n\nModule C1 | Deconstruction and demolition\nFor the disassembly of the mineral wool products, a manual dismantling was assumed. Referring energy demand is considered to be negligible.\n\nModule C2 | Transport to disposal\nModule C2 includes the transport to waste treatment. In this case, transport by truck over a transport distance of 50 km is assumed. This corresponds to the recommendations according to EURIMA (2019).\n\nModule C3 | Waste processing\nThe declared scenario assumes landfilling of the mineral wool, therefore no environmental impacts from the waste treatment of the products are declared in C3. \n\nModule C4 | Disposal\nModule C4 refers to the emissions from the disposal of the insulation material. The chosen scenario, therefore, includes the environmental burdens of landfilling of the product. The biogenic carbon in the binder of the products is treated as emissions of biogenic CO2 from the technosphere into the natural environment.\n\nModule D | Benefits and loads beyond the system boundary\nIn module D the substitution potential from the energy recovery of the packaging is declared.", "lang": "en"}], "other": {"anies": [{"name": "referenceToOriginalEPD", "value": {"shortDescription": {"value": "Mineralwolle-Dämmstoff im niedrigen Rohdichtebereich.pdf", "defaultValue": "Mineralwolle-Dämmstoff im niedrigen Rohdichtebereich.pdf", "lstrings": [{"lang": "de", "value": "Mineralwolle-Dämmstoff im niedrigen Rohdichtebereich.pdf"}]}, "type": "source data set", "uuid": {"uuid": "215ee85c-8e2f-40fd-b775-794df531aa9d"}, "refObjectId": "215ee85c-8e2f-40fd-b775-794df531aa9d", "resourceURLs": ["https://oekobaudat.de/OEKOBAU.DAT/resource/sources/215ee85c-8e2f-40fd-b775-794df531aa9d/Mineralwolle-Daemmstoff_im_niedrigen_Rohdichtebereich_18233.pdf?version=00.02.000"]}}]}}, "validation": {"review": [{"referenceToNameOfReviewerAndInstitution": [{"shortDescription": [{"value": "Institut Bauen und Umwelt e. V.", "lang": "de"}], "type": "contact data set", "refObjectId": "d111dbec-b024-4be5-86c5-752d6eb2cf95", "uri": "../contacts/d111dbec-b024-4be5-86c5-752d6eb2cf95.xml"}], "type": "Accredited third party review"}]}, "complianceDeclarations": {"compliance": [{"referenceToComplianceSystem": {"shortDescription": [{"value": "DIN EN 15804+A2", "lang": "de"}], "type": "source data set", "refObjectId": "c0016b33-8cf7-415c-ac6e-deba0d21440d", "uri": "../sources/c0016b33-8cf7-415c-ac6e-deba0d21440d.xml"}}, {"referenceToComplianceSystem": {"shortDescription": [{"value": "ISO 14025", "lang": "de"}], "type": "source data set", "refObjectId": "4f2eb655-6e44-4874-a95a-e28f5442cd4d", "uri": "../sources/4f2eb655-6e44-4874-a95a-e28f5442cd4d.xml"}}]}}, "administrativeInformation": {"commissionerAndGoal": {"referenceToCommissioner": [{"shortDescription": [{"value": "FMI Fachverband Mineralwolleindustrie e.V.", "lang": "de"}], "type": "contact data set", "refObjectId": "964fbdfe-2345-49da-9588-91347ed0aa3d", "uri": "../contacts/964fbdfe-2345-49da-9588-91347ed0aa3d.xml"}]}, "dataGenerator": {"referenceToPersonOrEntityGeneratingTheDataSet": [{"shortDescription": [{"value": "Daxner & Merl GmbH", "lang": "de"}], "type": "contact data set", "refObjectId": "ad8ad627-3991-42b7-a7ca-5a3fe0a34c28", "uri": "../contacts/ad8ad627-3991-42b7-a7ca-5a3fe0a34c28.xml"}]}, "dataEntryBy": {"timeStamp": 1687996800000, "referenceToDataSetFormat": [{"shortDescription": [{"value": "ILCD Format", "lang": "de"}], "type": "source data set", "refObjectId": "a97a0155-0234-4b87-b4ce-a45da52f2a40", "uri": "../sources/a97a0155-0234-4b87-b4ce-a45da52f2a40.xml"}, {"shortDescription": [{"value": "EPD-Datenformaterweiterungen v1.2", "lang": "de"}, {"value": "EPD Data Format Extensions v1.2", "lang": "en"}], "type": "source data set", "refObjectId": "a29449fd-aa2f-4de8-b5d7-4b06b43c6fde", "uri": "../sources/a29449fd-aa2f-4de8-b5d7-4b06b43c6fde.xml"}]}, "publicationAndOwnership": {"dataSetVersion": "00.09.000", "referenceToRegistrationAuthority": {"shortDescription": [{"value": "Institut Bauen und Umwelt e. V.", "lang": "de"}], "type": "contact data set", "refObjectId": "d111dbec-b024-4be5-86c5-752d6eb2cf95", "uri": "../contacts/d111dbec-b024-4be5-86c5-752d6eb2cf95.xml"}, "registrationNumber": "EPD-FMI-20210016-IBG1-DE", "referenceToOwnershipOfDataSet": {"shortDescription": [{"value": "FMI Fachverband Mineralwolleindustrie e.V.", "lang": "de"}], "type": "contact data set", "refObjectId": "964fbdfe-2345-49da-9588-91347ed0aa3d", "uri": "../contacts/964fbdfe-2345-49da-9588-91347ed0aa3d.xml"}, "copyright": true, "licenseType": "Free of charge for all users and uses", "accessRestrictions": [{"value": "None", "lang": "en"}], "other": {"anies": [{"name": "referenceToPublisher", "value": {"shortDescription": [{"value": "Institut Bauen und Umwelt e. V.", "lang": "de"}], "type": "contact data set", "refObjectId": "d111dbec-b024-4be5-86c5-752d6eb2cf95", "uri": "../contacts/d111dbec-b024-4be5-86c5-752d6eb2cf95.xml"}}]}}}, "exchanges": {"exchange": [{"dataSetInternalID": 0, "referenceToFlowDataSet": {"shortDescription": [{"value": "Mineralwolle-Dämmstoff (Mineralwolle-Dämmstoff)", "lang": "de"}], "type": "flow data set", "refObjectId": "714d036a-58fb-3cdd-cc90-fffee1714c18", "uri": "../flows/714d036a-58fb-3cdd-cc90-fffee1714c18.xml"}, "meanAmount": 1.0, "referencesToDataSource": {}, "referenceFlow": true, "resolvedFlowVersion": "00.03.000", "resultingflowAmount": 1.0, "flowProperties": [{"name": [{"lang": "en", "value": "Volume"}, {"lang": "de", "value": "Volumen"}], "uuid": "93a60a56-a3c8-22da-a746-0800200c9a66", "referenceFlowProperty": true, "meanValue": 1.0, "referenceUnit": "m3", "unitGroupUUID": "cd950537-0a98-4044-9ba7-9f9a68d0a504"}], "materialProperties": [{"name": "gross density", "value": "24.0", "unit": "kg/m^3", "unitDescription": "kilograms per cubic metre"}], "typeOfFlow": "Product flow", "classification": {"classHierarchy": "Dämmstoffe / Mineralwolle / Mineralwolle", "name": "OEKOBAU.DAT"}}, {"dataSetInternalID": 1, "referenceToFlowDataSet": {"shortDescription": [{"value": "Erneuerbare Primärenergie als Energieträger (PERE)", "lang": "de"}, {"value": "Renewable primary energy as energy carrier (PERE)", "lang": "en"}], "type": "flow data set", "refObjectId": "20f32be5-0398-4288-9b6d-accddd195317", "uri": "../flows/20f32be5-0398-4288-9b6d-accddd195317.xml"}, "exchange direction": "INPUT", "other": {"anies": [{"name": "referenceToUnitGroupDataSet", "value": {"shortDescription": [{"value": "MJ", "lang": "de"}], "type": "unit group data set", "refObjectId": "93a60a57-a3c8-11da-a746-0800200c9a66", "uri": "../unitgroups/93a60a57-a3c8-11da-a746-0800200c9a66.xml"}}, {"value": "77.2248741561842", "module": "A1-A3"}, {"value": "0.400547621389403", "module": "A4"}, {"value": "27.0593165477386", "module": "A5"}, {"value": "0.0556316140818616", "module": "C2"}, {"value": "0.625343954619649", "module": "C4"}, {"value": "-5.55361935001149", "module": "D"}]}, "resolvedFlowVersion": "38.00.000", "flowProperties": [], "typeOfFlow": "Other flow", "classification": {"classHierarchy": "Quantities", "name": "GaBiCategories"}}, {"dataSetInternalID": 2, "referenceToFlowDataSet": {"shortDescription": [{"value": "Erneuerbare Primärenergie zur stofflichen Nutzung (PERM)", "lang": "de"}, {"value": "Renewable primary energy resources as material utilization (PERM)", "lang": "en"}], "type": "flow data set", "refObjectId": "fb3ec0de-548d-4508-aea5-00b73bf6f702", "uri": "../flows/fb3ec0de-548d-4508-aea5-00b73bf6f702.xml"}, "exchange direction": "INPUT", "other": {"anies": [{"name": "referenceToUnitGroupDataSet", "value": {"shortDescription": [{"value": "MJ", "lang": "de"}], "type": "unit group data set", "refObjectId": "93a60a57-a3c8-11da-a746-0800200c9a66", "uri": "../unitgroups/93a60a57-a3c8-11da-a746-0800200c9a66.xml"}}, {"value": "45.0811893013148", "module": "A1-A3"}, {"value": "0", "module": "A4"}, {"value": "-24.4640101197", "module": "A5"}, {"value": "0", "module": "C2"}, {"value": "0", "module": "C4"}, {"value": "0", "module": "D"}]}, "resolvedFlowVersion": "38.00.000", "flowProperties": [], "typeOfFlow": "Other flow", "classification": {"classHierarchy": "Quantities", "name": "GaBiCategories"}}, {"dataSetInternalID": 3, "referenceToFlowDataSet": {"shortDescription": [{"value": "Total erneuerbare Primärenergie (PERT)", "lang": "de"}, {"value": "Total use of renewable primary energy resources (PERT)", "lang": "en"}], "type": "flow data set", "refObjectId": "53f97275-fa8a-4cdd-9024-65936002acd0", "uri": "../flows/53f97275-fa8a-4cdd-9024-65936002acd0.xml"}, "exchange direction": "INPUT", "other": {"anies": [{"name": "referenceToUnitGroupDataSet", "value": {"shortDescription": [{"value": "MJ", "lang": "de"}], "type": "unit group data set", "refObjectId": "93a60a57-a3c8-11da-a746-0800200c9a66", "uri": "../unitgroups/93a60a57-a3c8-11da-a746-0800200c9a66.xml"}}, {"value": "122.306063457499", "module": "A1-A3"}, {"value": "0.400547621389403", "module": "A4"}, {"value": "2.59530642803863", "module": "A5"}, {"value": "0.0556316140818616", "module": "C2"}, {"value": "0.625343954619649", "module": "C4"}, {"value": "-5.55361935001149", "module": "D"}]}, "resolvedFlowVersion": "38.00.000", "flowProperties": [], "typeOfFlow": "Other flow", "classification": {"classHierarchy": "Quantities / Environmental quantities / EPD EN 15804 / LCI indicators", "name": "GaBiCategories"}}, {"dataSetInternalID": 4, "referenceToFlowDataSet": {"shortDescription": [{"value": "Nicht-erneuerbare Primärenergie als Energieträger (PENRE)", "lang": "de"}, {"value": "Non renewable primary energy as energy carrier (PENRE)", "lang": "en"}], "type": "flow data set", "refObjectId": "ac857178-2b45-46ec-892a-a9a4332f0372", "uri": "../flows/ac857178-2b45-46ec-892a-a9a4332f0372.xml"}, "exchange direction": "INPUT", "other": {"anies": [{"name": "referenceToUnitGroupDataSet", "value": {"shortDescription": [{"value": "MJ", "lang": "de"}], "type": "unit group data set", "refObjectId": "93a60a57-a3c8-11da-a746-0800200c9a66", "uri": "../unitgroups/93a60a57-a3c8-11da-a746-0800200c9a66.xml"}}, {"value": "507.376737619614", "module": "A1-A3"}, {"value": "6.95519066253132", "module": "A4"}, {"value": "29.6968135338027", "module": "A5"}, {"value": "0.96599870312935", "module": "C2"}, {"value": "4.7780338201199", "module": "C4"}, {"value": "-25.2962613874741", "module": "D"}]}, "resolvedFlowVersion": "38.00.000", "flowProperties": [], "typeOfFlow": "Other flow", "classification": {"classHierarchy": "Quantities", "name": "GaBiCategories"}}, {"dataSetInternalID": 5, "referenceToFlowDataSet": {"shortDescription": [{"value": "Nicht-erneuerbare Primärenergie zur stofflichen Nutzung (PENRM)", "lang": "de"}, {"value": "Non renewable primary energy as material utilization (PENRM)", "lang": "en"}], "type": "flow data set", "refObjectId": "1421caa0-679d-4bf4-b282-0eb850ccae27", "uri": "../flows/1421caa0-679d-4bf4-b282-0eb850ccae27.xml"}, "exchange direction": "INPUT", "other": {"anies": [{"name": "referenceToUnitGroupDataSet", "value": {"shortDescription": [{"value": "MJ", "lang": "de"}], "type": "unit group data set", "refObjectId": "93a60a57-a3c8-11da-a746-0800200c9a66", "uri": "../unitgroups/93a60a57-a3c8-11da-a746-0800200c9a66.xml"}}, {"value": "51.1829740889577", "module": "A1-A3"}, {"value": "0", "module": "A4"}, {"value": "-17.5895186923162", "module": "A5"}, {"value": "0", "module": "C2"}, {"value": "0", "module": "C4"}, {"value": "0", "module": "D"}]}, "resolvedFlowVersion": "38.00.000", "flowProperties": [], "typeOfFlow": "Other flow", "classification": {"classHierarchy": "Quantities", "name": "GaBiCategories"}}, {"dataSetInternalID": 6, "referenceToFlowDataSet": {"shortDescription": [{"value": "Total nicht erneuerbare Primärenergie (PENRT)", "lang": "de"}, {"value": "Total use of non renewable primary energy resources (PENRT)", "lang": "en"}], "type": "flow data set", "refObjectId": "06159210-646b-4c8d-8583-da9b3b95a6c1", "uri": "../flows/06159210-646b-4c8d-8583-da9b3b95a6c1.xml"}, "exchange direction": "INPUT", "other": {"anies": [{"name": "referenceToUnitGroupDataSet", "value": {"shortDescription": [{"value": "MJ", "lang": "de"}], "type": "unit group data set", "refObjectId": "93a60a57-a3c8-11da-a746-0800200c9a66", "uri": "../unitgroups/93a60a57-a3c8-11da-a746-0800200c9a66.xml"}}, {"value": "558.559711708572", "module": "A1-A3"}, {"value": "6.95519066254335", "module": "A4"}, {"value": "12.1072948414865", "module": "A5"}, {"value": "0.965998703131021", "module": "C2"}, {"value": "4.77803382012414", "module": "C4"}, {"value": "-25.2962613874934", "module": "D"}]}, "resolvedFlowVersion": "38.00.000", "flowProperties": [], "typeOfFlow": "Other flow", "classification": {"classHierarchy": "Quantities / Environmental quantities / EPD EN 15804 / LCI indicators", "name": "GaBiCategories"}}, {"dataSetInternalID": 7, "referenceToFlowDataSet": {"shortDescription": [{"value": "Einsatz von Sekundärstoffen (SM)", "lang": "de"}, {"value": "Use of secondary material (SM)", "lang": "en"}], "type": "flow data set", "refObjectId": "c6a1f35f-2d09-4f54-8dfb-97e502e1ce92", "uri": "../flows/c6a1f35f-2d09-4f54-8dfb-97e502e1ce92.xml"}, "exchange direction": "INPUT", "other": {"anies": [{"name": "referenceToUnitGroupDataSet", "value": {"shortDescription": [{"value": "kg", "lang": "de"}], "type": "unit group data set", "refObjectId": "ad38d542-3fe9-439d-9b95-2f5f7752acaf", "uri": "../unitgroups/ad38d542-3fe9-439d-9b95-2f5f7752acaf.xml"}}, {"value": "11.1653198829726", "module": "A1-A3"}, {"value": "0", "module": "A4"}, {"value": "0.223306397659452", "module": "A5"}, {"value": "0", "module": "C2"}, {"value": "0", "module": "C4"}, {"value": "0", "module": "D"}]}, "resolvedFlowVersion": "38.00.000", "flowProperties": [], "typeOfFlow": "Other flow", "classification": {"classHierarchy": "Quantities / Environmental quantities / EPD EN 15804 / LCI indicators", "name": "GaBiCategories"}}, {"dataSetInternalID": 8, "referenceToFlowDataSet": {"shortDescription": [{"value": "Erneuerbare Sekundärbrennstoffe (RSF)", "lang": "de"}, {"value": "Use of renewable secondary fuels (RSF)", "lang": "en"}], "type": "flow data set", "refObjectId": "64333088-a55f-4aa2-9a31-c10b07816787", "uri": "../flows/64333088-a55f-4aa2-9a31-c10b07816787.xml"}, "exchange direction": "INPUT", "other": {"anies": [{"name": "referenceToUnitGroupDataSet", "value": {"shortDescription": [{"value": "MJ", "lang": "de"}], "type": "unit group data set", "refObjectId": "93a60a57-a3c8-11da-a746-0800200c9a66", "uri": "../unitgroups/93a60a57-a3c8-11da-a746-0800200c9a66.xml"}}, {"value": "0", "module": "A1-A3"}, {"value": "0", "module": "A4"}, {"value": "0", "module": "A5"}, {"value": "0", "module": "C2"}, {"value": "0", "module": "C4"}, {"value": "0", "module": "D"}]}, "resolvedFlowVersion": "38.00.000", "flowProperties": [], "typeOfFlow": "Other flow", "classification": {"classHierarchy": "Quantities / Environmental quantities / EPD EN 15804 / LCI indicators", "name": "GaBiCategories"}}, {"dataSetInternalID": 9, "referenceToFlowDataSet": {"shortDescription": [{"value": "Nicht erneuerbare Sekundärbrennstoffe (NRSF)", "lang": "de"}, {"value": "Use of non renewable secondary fuels (NRSF)", "lang": "en"}], "type": "flow data set", "refObjectId": "89def144-d39a-4287-b86f-efde453ddcb2", "uri": "../flows/89def144-d39a-4287-b86f-efde453ddcb2.xml"}, "exchange direction": "INPUT", "other": {"anies": [{"name": "referenceToUnitGroupDataSet", "value": {"shortDescription": [{"value": "MJ", "lang": "de"}], "type": "unit group data set", "refObjectId": "93a60a57-a3c8-11da-a746-0800200c9a66", "uri": "../unitgroups/93a60a57-a3c8-11da-a746-0800200c9a66.xml"}}, {"value": "0", "module": "A1-A3"}, {"value": "0", "module": "A4"}, {"value": "0.0451660414325298", "module": "A5"}, {"value": "0", "module": "C2"}, {"value": "0", "module": "C4"}, {"value": "0", "module": "D"}]}, "resolvedFlowVersion": "38.00.000", "flowProperties": [], "typeOfFlow": "Other flow", "classification": {"classHierarchy": "Quantities / Environmental quantities / EPD EN 15804 / LCI indicators", "name": "GaBiCategories"}}, {"dataSetInternalID": 10, "referenceToFlowDataSet": {"shortDescription": [{"value": "Einsatz von Süßwasserressourcen (FW)", "lang": "de"}, {"value": "Use of net fresh water (FW)", "lang": "en"}], "type": "flow data set", "refObjectId": "3cf952c8-f3a4-461d-8c96-96456ca62246", "uri": "../flows/3cf952c8-f3a4-461d-8c96-96456ca62246.xml"}, "exchange direction": "INPUT", "other": {"anies": [{"name": "referenceToUnitGroupDataSet", "value": {"shortDescription": [{"value": "m^3", "lang": "de"}], "type": "unit group data set", "refObjectId": "cd950537-0a98-4044-9ba7-9f9a68d0a504", "uri": "../unitgroups/cd950537-0a98-4044-9ba7-9f9a68d0a504.xml"}}, {"value": "0.130913252606842", "module": "A1-A3"}, {"value": "0.00046677284717998", "module": "A4"}, {"value": "0.0114165823687957", "module": "A5"}, {"value": "6.48295621083297E-05", "module": "C2"}, {"value": "0.00120433838101075", "module": "C4"}, {"value": "-0.0064310845352642", "module": "D"}]}, "resolvedFlowVersion": "38.00.000", "flowProperties": [], "typeOfFlow": "Other flow", "classification": {"classHierarchy": "Quantities / Environmental quantities / EPD EN 15804 / LCI indicators", "name": "GaBiCategories"}}, {"dataSetInternalID": 11, "referenceToFlowDataSet": {"shortDescription": [{"value": "Gefährlicher Abfall zur Deponie (HWD)", "lang": "de"}, {"value": "Hazardous waste disposed (HWD)", "lang": "en"}], "type": "flow data set", "refObjectId": "430f9e0f-59b2-46a0-8e0d-55e0e84948fc", "uri": "../flows/430f9e0f-59b2-46a0-8e0d-55e0e84948fc.xml"}, "exchange direction": "OUTPUT", "other": {"anies": [{"name": "referenceToUnitGroupDataSet", "value": {"shortDescription": [{"value": "kg", "lang": "de"}], "type": "unit group data set", "refObjectId": "ad38d542-3fe9-439d-9b95-2f5f7752acaf", "uri": "../unitgroups/ad38d542-3fe9-439d-9b95-2f5f7752acaf.xml"}}, {"value": "1.67014969267061E-06", "module": "A1-A3"}, {"value": "3.21619331280559E-07", "module": "A4"}, {"value": "4.26572748592689E-08", "module": "A5"}, {"value": "4.46693515667443E-08", "module": "C2"}, {"value": "7.2831801141139E-08", "module": "C4"}, {"value": "-1.008963762801E-08", "module": "D"}]}, "resolvedFlowVersion": "38.00.000", "flowProperties": [], "typeOfFlow": "Other flow", "classification": {"classHierarchy": "Quantities / Environmental quantities / EPD EN 15804 / LCI indicators", "name": "GaBiCategories"}}, {"dataSetInternalID": 12, "referenceToFlowDataSet": {"shortDescription": [{"value": "Entsorgter nicht gefährlicher Abfall (NHWD)", "lang": "de"}, {"value": "Non hazardous waste disposed (NHWD)", "lang": "en"}], "type": "flow data set", "refObjectId": "b29ef66b-e286-4afa-949f-62f1a7b4d7fa", "uri": "../flows/b29ef66b-e286-4afa-949f-62f1a7b4d7fa.xml"}, "exchange direction": "OUTPUT", "other": {"anies": [{"name": "referenceToUnitGroupDataSet", "value": {"shortDescription": [{"value": "kg", "lang": "de"}], "type": "unit group data set", "refObjectId": "ad38d542-3fe9-439d-9b95-2f5f7752acaf", "uri": "../unitgroups/ad38d542-3fe9-439d-9b95-2f5f7752acaf.xml"}}, {"value": "3.9825759505743", "module": "A1-A3"}, {"value": "0.00110234398428472", "module": "A4"}, {"value": "0.582713552276898", "module": "A5"}, {"value": "0.000153103331150656", "module": "C2"}, {"value": "24.0237046508669", "module": "C4"}, {"value": "-0.0117200871429864", "module": "D"}]}, "resolvedFlowVersion": "38.00.000", "flowProperties": [], "typeOfFlow": "Other flow", "classification": {"classHierarchy": "Quantities / Environmental quantities / EPD EN 15804 / LCI indicators", "name": "GaBiCategories"}}, {"dataSetInternalID": 13, "referenceToFlowDataSet": {"shortDescription": [{"value": "Entsorgter radioaktiver Abfall (RWD)", "lang": "de"}, {"value": "Radioactive waste disposed (RWD)", "lang": "en"}], "type": "flow data set", "refObjectId": "3449546e-52ad-4b39-b809-9fb77cea8ff6", "uri": "../flows/3449546e-52ad-4b39-b809-9fb77cea8ff6.xml"}, "exchange direction": "OUTPUT", "other": {"anies": [{"name": "referenceToUnitGroupDataSet", "value": {"shortDescription": [{"value": "kg", "lang": "de"}], "type": "unit group data set", "refObjectId": "ad38d542-3fe9-439d-9b95-2f5f7752acaf", "uri": "../unitgroups/ad38d542-3fe9-439d-9b95-2f5f7752acaf.xml"}}, {"value": "0.014556975561652", "module": "A1-A3"}, {"value": "1.28190774281421E-05", "module": "A4"}, {"value": "0.000331756727028624", "module": "A5"}, {"value": "1.78042742057529E-06", "module": "C2"}, {"value": "5.42708525973658E-05", "module": "C4"}, {"value": "-0.00189656858413656", "module": "D"}]}, "resolvedFlowVersion": "38.00.000", "flowProperties": [], "typeOfFlow": "Other flow", "classification": {"classHierarchy": "Quantities / Environmental quantities / EPD EN 15804 / LCI indicators", "name": "GaBiCategories"}}, {"dataSetInternalID": 14, "referenceToFlowDataSet": {"shortDescription": [{"value": "Komponenten für die Wiederverwendung (CRU)", "lang": "de"}, {"value": "Components for re-use (CRU)", "lang": "en"}], "type": "flow data set", "refObjectId": "a2b32f97-3fc7-4af2-b209-525bc6426f33", "uri": "../flows/a2b32f97-3fc7-4af2-b209-525bc6426f33.xml"}, "exchange direction": "OUTPUT", "other": {"anies": [{"name": "referenceToUnitGroupDataSet", "value": {"shortDescription": [{"value": "kg", "lang": "de"}], "type": "unit group data set", "refObjectId": "ad38d542-3fe9-439d-9b95-2f5f7752acaf", "uri": "../unitgroups/ad38d542-3fe9-439d-9b95-2f5f7752acaf.xml"}}, {"value": "0", "module": "A1-A3"}, {"value": "0", "module": "A4"}, {"value": "0", "module": "A5"}, {"value": "0", "module": "C2"}, {"value": "0", "module": "C4"}, {"value": "0", "module": "D"}]}, "resolvedFlowVersion": "38.00.000", "flowProperties": [], "typeOfFlow": "Other flow", "classification": {"classHierarchy": "Quantities / Environmental quantities / EPD EN 15804 / LCI indicators", "name": "GaBiCategories"}}, {"dataSetInternalID": 15, "referenceToFlowDataSet": {"shortDescription": [{"value": "Stoffe zum Recycling (MFR)", "lang": "de"}, {"value": "Materials for recycling (MFR)", "lang": "en"}], "type": "flow data set", "refObjectId": "d7fe48a5-4103-49c8-9aae-b0b5dfdbd6ae", "uri": "../flows/d7fe48a5-4103-49c8-9aae-b0b5dfdbd6ae.xml"}, "exchange direction": "OUTPUT", "other": {"anies": [{"name": "referenceToUnitGroupDataSet", "value": {"shortDescription": [{"value": "kg", "lang": "de"}], "type": "unit group data set", "refObjectId": "ad38d542-3fe9-439d-9b95-2f5f7752acaf", "uri": "../unitgroups/ad38d542-3fe9-439d-9b95-2f5f7752acaf.xml"}}, {"value": "0", "module": "A1-A3"}, {"value": "0", "module": "A4"}, {"value": "0.0583813096510527", "module": "A5"}, {"value": "0", "module": "C2"}, {"value": "0", "module": "C4"}, {"value": "0", "module": "D"}]}, "resolvedFlowVersion": "38.00.000", "flowProperties": [], "typeOfFlow": "Other flow", "classification": {"classHierarchy": "Quantities / Environmental quantities / EPD EN 15804 / LCI indicators", "name": "GaBiCategories"}}, {"dataSetInternalID": 16, "referenceToFlowDataSet": {"shortDescription": [{"value": "Stoffe für die Energierückgewinnung (MER)", "lang": "de"}, {"value": "Materials for energy recovery (MER)", "lang": "en"}], "type": "flow data set", "refObjectId": "59a9181c-3aaf-46ee-8b13-2b3723b6e447", "uri": "../flows/59a9181c-3aaf-46ee-8b13-2b3723b6e447.xml"}, "exchange direction": "OUTPUT", "other": {"anies": [{"name": "referenceToUnitGroupDataSet", "value": {"shortDescription": [{"value": "kg", "lang": "de"}], "type": "unit group data set", "refObjectId": "ad38d542-3fe9-439d-9b95-2f5f7752acaf", "uri": "../unitgroups/ad38d542-3fe9-439d-9b95-2f5f7752acaf.xml"}}, {"value": "0", "module": "A1-A3"}, {"value": "0", "module": "A4"}, {"value": "0", "module": "A5"}, {"value": "0", "module": "C2"}, {"value": "0", "module": "C4"}, {"value": "0", "module": "D"}]}, "resolvedFlowVersion": "38.00.000", "flowProperties": [], "typeOfFlow": "Other flow", "classification": {"classHierarchy": "Quantities / Environmental quantities / EPD EN 15804 / LCI indicators", "name": "GaBiCategories"}}, {"dataSetInternalID": 17, "referenceToFlowDataSet": {"shortDescription": [{"value": "Exportierte elektrische Energie (EEE)", "lang": "de"}, {"value": "Exported electrical energy (EEE)", "lang": "en"}], "type": "flow data set", "refObjectId": "4da0c987-2b76-40d6-9e9e-82a017aaaf29", "uri": "../flows/4da0c987-2b76-40d6-9e9e-82a017aaaf29.xml"}, "exchange direction": "OUTPUT", "other": {"anies": [{"name": "referenceToUnitGroupDataSet", "value": {"shortDescription": [{"value": "MJ", "lang": "de"}], "type": "unit group data set", "refObjectId": "93a60a57-a3c8-11da-a746-0800200c9a66", "uri": "../unitgroups/93a60a57-a3c8-11da-a746-0800200c9a66.xml"}}, {"value": "0", "module": "A1-A3"}, {"value": "0", "module": "A4"}, {"value": "6.34517737848709", "module": "A5"}, {"value": "0", "module": "C2"}, {"value": "0", "module": "C4"}, {"value": "0", "module": "D"}]}, "resolvedFlowVersion": "38.00.000", "flowProperties": [], "typeOfFlow": "Other flow", "classification": {"classHierarchy": "Quantities / Environmental quantities / EPD EN 15804 / LCI indicators", "name": "GaBiCategories"}}, {"dataSetInternalID": 18, "referenceToFlowDataSet": {"shortDescription": [{"value": "Exportierte thermische Energie (EET)", "lang": "de"}, {"value": "Exported thermal energy (EET)", "lang": "en"}], "type": "flow data set", "refObjectId": "98daf38a-7a79-46d3-9a37-2b7bd0955810", "uri": "../flows/98daf38a-7a79-46d3-9a37-2b7bd0955810.xml"}, "exchange direction": "OUTPUT", "other": {"anies": [{"name": "referenceToUnitGroupDataSet", "value": {"shortDescription": [{"value": "MJ", "lang": "de"}], "type": "unit group data set", "refObjectId": "93a60a57-a3c8-11da-a746-0800200c9a66", "uri": "../unitgroups/93a60a57-a3c8-11da-a746-0800200c9a66.xml"}}, {"value": "0", "module": "A1-A3"}, {"value": "0", "module": "A4"}, {"value": "11.3446836077137", "module": "A5"}, {"value": "0", "module": "C2"}, {"value": "0", "module": "C4"}, {"value": "0", "module": "D"}]}, "resolvedFlowVersion": "38.00.000", "flowProperties": [], "typeOfFlow": "Other flow", "classification": {"classHierarchy": "Quantities / Environmental quantities / EPD EN 15804 / LCI indicators", "name": "GaBiCategories"}}]}, "LCIAResults": {"LCIAResult": [{"referenceToLCIAMethodDataSet": {"shortDescription": [{"value": "Globales Erwärmungspotenzial total (GWP-total)", "lang": "de"}, {"value": "Global Warming Potential total (GWP-total)", "lang": "en"}], "type": "LCIA method data set", "refObjectId": "6a37f984-a4b3-458a-a20a-64418c145fa2", "uri": "../lciamethods/6a37f984-a4b3-458a-a20a-64418c145fa2.xml"}, "other": {"anies": [{"name": "referenceToUnitGroupDataSet", "value": {"shortDescription": [{"value": "kg CO_(2)-Äq.", "lang": "de"}], "type": "unit group data set", "refObjectId": "1ebf3012-d0db-4de2-aefd-ef30cedb0be1", "uri": "../unitgroups/1ebf3012-d0db-4de2-aefd-ef30cedb0be1.xml"}}, {"value": "34.4900480386392", "module": "A1-A3"}, {"value": "0.52400534569911", "module": "A4"}, {"value": "4.58614547985493", "module": "A5"}, {"value": "0.0727785202359874", "module": "C2"}, {"value": "1.51700514646619", "module": "C4"}, {"value": "-1.49550780862089", "module": "D"}]}}, {"referenceToLCIAMethodDataSet": {"shortDescription": [{"value": "Globales Erwärmungspotenzial fossil (GWP-fossil)", "lang": "de"}, {"value": "Global Warming Potential fossil fuels (GWP-fossil)", "lang": "en"}], "type": "LCIA method data set", "refObjectId": "5f635281-343e-44fb-83df-1971b155e6b6", "uri": "../lciamethods/5f635281-343e-44fb-83df-1971b155e6b6.xml"}, "other": {"anies": [{"name": "referenceToUnitGroupDataSet", "value": {"shortDescription": [{"value": "kg CO_(2)-Äq.", "lang": "de"}], "type": "unit group data set", "refObjectId": "1ebf3012-d0db-4de2-aefd-ef30cedb0be1", "uri": "../unitgroups/1ebf3012-d0db-4de2-aefd-ef30cedb0be1.xml"}}, {"value": "38.2308529525192", "module": "A1-A3"}, {"value": "0.520674282634743", "module": "A4"}, {"value": "2.16631240586954", "module": "A5"}, {"value": "0.0723158725881588", "module": "C2"}, {"value": "0.364014243939195", "module": "C4"}, {"value": "-1.49094954374604", "module": "D"}]}}, {"referenceToLCIAMethodDataSet": {"shortDescription": [{"value": "Globales Erwärmungspotenzial biogen (GWP-biogenic)", "lang": "de"}, {"value": "Global Warming Potential biogenic (GWP-biogenic)", "lang": "en"}], "type": "LCIA method data set", "refObjectId": "2356e1ab-0185-4db5-86e5-16de51c7485c", "uri": "../lciamethods/2356e1ab-0185-4db5-86e5-16de51c7485c.xml"}, "other": {"anies": [{"name": "referenceToUnitGroupDataSet", "value": {"shortDescription": [{"value": "kg CO_(2)-Äq.", "lang": "de"}], "type": "unit group data set", "refObjectId": "1ebf3012-d0db-4de2-aefd-ef30cedb0be1", "uri": "../unitgroups/1ebf3012-d0db-4de2-aefd-ef30cedb0be1.xml"}}, {"value": "-3.77918270619954", "module": "A1-A3"}, {"value": "-0.000871622070743844", "module": "A4"}, {"value": "2.41891829690414", "module": "A5"}, {"value": "-0.000121058620936644", "module": "C2"}, {"value": "1.1519431847804", "module": "C4"}, {"value": "-0.00350887920592324", "module": "D"}]}}, {"referenceToLCIAMethodDataSet": {"shortDescription": [{"value": "Globales Erwärmungspotenzial luluc (GWP-luluc)", "lang": "de"}, {"value": "Global Warming Potential luluc (GWP-luluc)", "lang": "en"}], "type": "LCIA method data set", "refObjectId": "4331bbdb-978a-490d-8707-eeb047f01a55", "uri": "../lciamethods/4331bbdb-978a-490d-8707-eeb047f01a55.xml"}, "other": {"anies": [{"name": "referenceToUnitGroupDataSet", "value": {"shortDescription": [{"value": "kg CO_(2)-Äq.", "lang": "de"}], "type": "unit group data set", "refObjectId": "1ebf3012-d0db-4de2-aefd-ef30cedb0be1", "uri": "../unitgroups/1ebf3012-d0db-4de2-aefd-ef30cedb0be1.xml"}}, {"value": "0.0383777923195462", "module": "A1-A3"}, {"value": "0.0042026851351099", "module": "A4"}, {"value": "0.000914777081248503", "module": "A5"}, {"value": "0.000583706268765264", "module": "C2"}, {"value": "0.00104771774659615", "module": "C4"}, {"value": "-0.00104938566892809", "module": "D"}]}}, {"referenceToLCIAMethodDataSet": {"shortDescription": [{"value": "Abbau Potential der stratosphärischen Ozonschicht (ODP)", "lang": "de"}, {"value": "Depletion potential of the stratospheric ozone layer (ODP)", "lang": "en"}], "type": "LCIA method data set", "refObjectId": "b5c629d6-def3-11e6-bf01-fe55135034f3", "uri": "../lciamethods/b5c629d6-def3-11e6-bf01-fe55135034f3.xml"}, "other": {"anies": [{"name": "referenceToUnitGroupDataSet", "value": {"shortDescription": [{"value": "kg CFC11-Äq.", "lang": "de"}], "type": "unit group data set", "refObjectId": "d9e957c9-7309-4474-bf3a-7777df6c4e5b", "uri": "../unitgroups/d9e957c9-7309-4474-bf3a-7777df6c4e5b.xml"}}, {"value": "1.24695227776724E-10", "module": "A1-A3"}, {"value": "9.52922385155623E-17", "module": "A4"}, {"value": "2.49432186823772E-12", "module": "A5"}, {"value": "1.32350331271614E-17", "module": "C2"}, {"value": "1.34897243350021E-15", "module": "C4"}, {"value": "-1.56450887599557E-14", "module": "D"}]}}, {"referenceToLCIAMethodDataSet": {"shortDescription": [{"value": "Versauerungspotenzial von Boden und Wasser (AP)", "lang": "de"}, {"value": "Acidification potential of land and water (AP)", "lang": "en"}], "type": "LCIA method data set", "refObjectId": "b5c611c6-def3-11e6-bf01-fe55135034f3", "uri": "../lciamethods/b5c611c6-def3-11e6-bf01-fe55135034f3.xml"}, "other": {"anies": [{"name": "referenceToUnitGroupDataSet", "value": {"shortDescription": [{"value": "mol H^(+)-Äq.", "lang": "de"}], "type": "unit group data set", "refObjectId": "42e089ac-92bf-4bf2-8ca1-5fc40d18f2ed", "uri": "../unitgroups/42e089ac-92bf-4bf2-8ca1-5fc40d18f2ed.xml"}}, {"value": "0.289920873584893", "module": "A1-A3"}, {"value": "0.00106453545005435", "module": "A4"}, {"value": "0.00635616214923843", "module": "A5"}, {"value": "0.000147852145840881", "module": "C2"}, {"value": "0.00261161127203043", "module": "C4"}, {"value": "-0.00209363858016587", "module": "D"}]}}, {"referenceToLCIAMethodDataSet": {"shortDescription": [{"value": "Eutrophierungspotenzial Süßwasser (EP-freshwater)", "lang": "de"}, {"value": "Eutrophication potential aquatic freshwater (EP-freshwater)", "lang": "en"}], "type": "LCIA method data set", "refObjectId": "b53ec18f-7377-4ad3-86eb-cc3f4f276b2b", "uri": "../lciamethods/b53ec18f-7377-4ad3-86eb-cc3f4f276b2b.xml"}, "other": {"anies": [{"name": "referenceToUnitGroupDataSet", "value": {"shortDescription": [{"value": "kg P-Äq.", "lang": "de"}], "type": "unit group data set", "refObjectId": "0429039d-a61d-4590-ba67-aa4a20a810a1", "uri": "../unitgroups/0429039d-a61d-4590-ba67-aa4a20a810a1.xml"}}, {"value": "0.000460970363122565", "module": "A1-A3"}, {"value": "1.58144844478233E-06", "module": "A4"}, {"value": "9.32525857297568E-06", "module": "A5"}, {"value": "2.19645617330878E-07", "module": "C2"}, {"value": "6.2517553718012E-07", "module": "C4"}, {"value": "-1.93254588574342E-06", "module": "D"}]}}, {"referenceToLCIAMethodDataSet": {"shortDescription": [{"value": "Eutrophierungspotenzial Salzwasser (EP-marine)", "lang": "de"}, {"value": "Eutrophication potential aquatic marine (EP-marine)", "lang": "en"}], "type": "LCIA method data set", "refObjectId": "b5c619fa-def3-11e6-bf01-fe55135034f3", "uri": "../lciamethods/b5c619fa-def3-11e6-bf01-fe55135034f3.xml"}, "other": {"anies": [{"name": "referenceToUnitGroupDataSet", "value": {"shortDescription": [{"value": "kg N-Äq.", "lang": "de"}], "type": "unit group data set", "refObjectId": "d05bb823-ecdf-4686-8c40-bf1d9257859f", "uri": "../unitgroups/d05bb823-ecdf-4686-8c40-bf1d9257859f.xml"}}, {"value": "0.0367718817603668", "module": "A1-A3"}, {"value": "0.000428368503364449", "module": "A4"}, {"value": "0.000899351040184427", "module": "A5"}, {"value": "5.94956254672846E-05", "module": "C2"}, {"value": "0.000672171462493573", "module": "C4"}, {"value": "-0.000540895557025323", "module": "D"}]}}, {"referenceToLCIAMethodDataSet": {"shortDescription": [{"value": "Eutrophierungspotenzial Land (EP-terrestrial)", "lang": "de"}, {"value": "Eutrophication potential terrestrial (EP-terrestrial)", "lang": "en"}], "type": "LCIA method data set", "refObjectId": "b5c614d2-def3-11e6-bf01-fe55135034f3", "uri": "../lciamethods/b5c614d2-def3-11e6-bf01-fe55135034f3.xml"}, "other": {"anies": [{"name": "referenceToUnitGroupDataSet", "value": {"shortDescription": [{"value": "mol N-Äq.", "lang": "de"}], "type": "unit group data set", "refObjectId": "71b4d617-0ec9-4d3f-b65e-e438940c2401", "uri": "../unitgroups/71b4d617-0ec9-4d3f-b65e-e438940c2401.xml"}}, {"value": "1.09246675381363", "module": "A1-A3"}, {"value": "0.00486256483591682", "module": "A4"}, {"value": "0.0243690728618139", "module": "A5"}, {"value": "0.000675356227210669", "module": "C2"}, {"value": "0.00738602043162681", "module": "C4"}, {"value": "-0.00579499376937094", "module": "D"}]}}, {"referenceToLCIAMethodDataSet": {"shortDescription": [{"value": "Bildungspotential für troposphärisches Ozon (POCP)", "lang": "de"}, {"value": "Formation potential of tropospheric ozone photochemical oxidants (POCP)", "lang": "en"}], "type": "LCIA method data set", "refObjectId": "b5c610fe-def3-11e6-bf01-fe55135034f3", "uri": "../lciamethods/b5c610fe-def3-11e6-bf01-fe55135034f3.xml"}, "other": {"anies": [{"name": "referenceToUnitGroupDataSet", "value": {"shortDescription": [{"value": "kg NMVOC-Äq.", "lang": "de"}], "type": "unit group data set", "refObjectId": "d27c25f8-fbc1-44c6-b47b-4adbae4199c6", "uri": "../unitgroups/d27c25f8-fbc1-44c6-b47b-4adbae4199c6.xml"}}, {"value": "0.0940373274095141", "module": "A1-A3"}, {"value": "0.000924014745922588", "module": "A4"}, {"value": "0.00233241939620667", "module": "A5"}, {"value": "0.000128335381378137", "module": "C2"}, {"value": "0.00203551456533949", "module": "C4"}, {"value": "-0.0015537656780043", "module": "D"}]}}, {"referenceToLCIAMethodDataSet": {"shortDescription": [{"value": "Potenzial für den abiotischen Abbau nicht fossiler Ressourcen (ADPE)", "lang": "de"}, {"value": "Abiotic depletion potential for non fossil resources (ADPE)", "lang": "en"}], "type": "LCIA method data set", "refObjectId": "b2ad6494-c78d-11e6-9d9d-cec0c932ce01", "uri": "../lciamethods/b2ad6494-c78d-11e6-9d9d-cec0c932ce01.xml"}, "other": {"anies": [{"name": "referenceToUnitGroupDataSet", "value": {"shortDescription": [{"value": "kg Sb-Äq.", "lang": "de"}], "type": "unit group data set", "refObjectId": "54ccd2d9-a32a-4fc2-923d-f2c8c93e89d4", "uri": "../unitgroups/54ccd2d9-a32a-4fc2-923d-f2c8c93e89d4.xml"}}, {"value": "2.4777157330329E-05", "module": "A1-A3"}, {"value": "4.19841017820077E-08", "module": "A4"}, {"value": "5.03315306520626E-07", "module": "A5"}, {"value": "5.83112524750106E-09", "module": "C2"}, {"value": "3.26865469220478E-08", "module": "C4"}, {"value": "-2.45635811108674E-07", "module": "D"}]}}, {"referenceToLCIAMethodDataSet": {"shortDescription": [{"value": "Potenzial für den abiotischen Abbau fossiler Brennstoffe (ADPF)", "lang": "de"}, {"value": "Abiotic depletion potential for fossil resources (ADPF)", "lang": "en"}], "type": "LCIA method data set", "refObjectId": "b2ad6110-c78d-11e6-9d9d-cec0c932ce01", "uri": "../lciamethods/b2ad6110-c78d-11e6-9d9d-cec0c932ce01.xml"}, "other": {"anies": [{"name": "referenceToUnitGroupDataSet", "value": {"shortDescription": [{"value": "MJ", "lang": "de"}], "type": "unit group data set", "refObjectId": "93a60a57-a3c8-11da-a746-0800200c9a66", "uri": "../unitgroups/93a60a57-a3c8-11da-a746-0800200c9a66.xml"}}, {"value": "558.293825515496", "module": "A1-A3"}, {"value": "6.92741679602153", "module": "A4"}, {"value": "12.1010411137005", "module": "A5"}, {"value": "0.962141221669657", "module": "C2"}, {"value": "4.77578653448457", "module": "C4"}, {"value": "-25.2936119705604", "module": "D"}]}}, {"referenceToLCIAMethodDataSet": {"shortDescription": [{"value": "Wassernutzung (WDP)", "lang": "de"}, {"value": "Water use (WDP)", "lang": "en"}], "type": "LCIA method data set", "refObjectId": "b2ad66ce-c78d-11e6-9d9d-cec0c932ce01", "uri": "../lciamethods/b2ad66ce-c78d-11e6-9d9d-cec0c932ce01.xml"}, "other": {"anies": [{"name": "referenceToUnitGroupDataSet", "value": {"shortDescription": [{"value": "m^(3) Welt-Äq. entzogen", "lang": "de"}], "type": "unit group data set", "refObjectId": "6ae2df01-888e-46c8-b17d-49fa3869b476", "uri": "../unitgroups/6ae2df01-888e-46c8-b17d-49fa3869b476.xml"}}, {"value": "0.426713213446533", "module": "A1-A3"}, {"value": "0.00506282251820656", "module": "A4"}, {"value": "0.382709290206221", "module": "A5"}, {"value": "0.000703169794195366", "module": "C2"}, {"value": "0.038153401494601", "module": "C4"}, {"value": "-0.155352801609176", "module": "D"}]}}, {"referenceToLCIAMethodDataSet": {"shortDescription": [{"value": "Auftreten von Krankheiten aufgrund von Feinstaubemissionen (PM)", "lang": "de"}, {"value": "Incidence of disease due to PM emissions (PM)", "lang": "en"}], "type": "LCIA method data set", "refObjectId": "b5c602c6-def3-11e6-bf01-fe55135034f3", "uri": "../lciamethods/b5c602c6-def3-11e6-bf01-fe55135034f3.xml"}, "other": {"anies": [{"name": "referenceToUnitGroupDataSet", "value": {"shortDescription": [{"value": "Krankheitsfälle", "lang": "de"}], "type": "unit group data set", "refObjectId": "3883559b-648f-4afc-8ba2-0bd24f3affa3", "uri": "../unitgroups/3883559b-648f-4afc-8ba2-0bd24f3affa3.xml"}}, {"module": "A1-A3"}, {"module": "A4"}, {"module": "A5"}, {"module": "C2"}, {"module": "C4"}, {"module": "D"}]}}, {"referenceToLCIAMethodDataSet": {"shortDescription": [{"value": "Wirkung durch Exposition des Menschen mit U235 (IR)", "lang": "de"}, {"value": "Human exposure efficiency relative to U235 (IR)", "lang": "en"}], "type": "LCIA method data set", "refObjectId": "b5c632be-def3-11e6-bf01-fe55135034f3", "uri": "../lciamethods/b5c632be-def3-11e6-bf01-fe55135034f3.xml"}, "other": {"anies": [{"name": "referenceToUnitGroupDataSet", "value": {"shortDescription": [{"value": "kBq U235-Äq.", "lang": "de"}], "type": "unit group data set", "refObjectId": "456b05bf-1415-44a9-9993-02452f554c09", "uri": "../unitgroups/456b05bf-1415-44a9-9993-02452f554c09.xml"}}, {"module": "A1-A3"}, {"module": "A4"}, {"module": "A5"}, {"module": "C2"}, {"module": "C4"}, {"module": "D"}]}}, {"referenceToLCIAMethodDataSet": {"shortDescription": [{"value": "Toxizitätsvergleichseinheit für Ökosysteme (ETP-fw)", "lang": "de"}, {"value": "Comparative toxic unit for ecosystems (ETP-fw)", "lang": "en"}], "type": "LCIA method data set", "refObjectId": "ee1082d1-b0f7-43ca-a1f0-21e2a4a74511", "uri": "../lciamethods/ee1082d1-b0f7-43ca-a1f0-21e2a4a74511.xml"}, "other": {"anies": [{"name": "referenceToUnitGroupDataSet", "value": {"shortDescription": [{"value": "CTUe", "lang": "de"}], "type": "unit group data set", "refObjectId": "aa959ded-f1eb-4efb-9c5c-2d60be36b3e6", "uri": "../unitgroups/aa959ded-f1eb-4efb-9c5c-2d60be36b3e6.xml"}}, {"module": "A1-A3"}, {"module": "A4"}, {"module": "A5"}, {"module": "C2"}, {"module": "C4"}, {"module": "D"}]}}, {"referenceToLCIAMethodDataSet": {"shortDescription": [{"value": "Toxizitätsvergleichseinheit für Menschen (krebserregend) (HTP-c)", "lang": "de"}, {"value": "Comparative toxic unit for humans (carcinogenic) (HTP-c)", "lang": "en"}], "type": "LCIA method data set", "refObjectId": "2299222a-bbd8-474f-9d4f-4dd1f18aea7c", "uri": "../lciamethods/2299222a-bbd8-474f-9d4f-4dd1f18aea7c.xml"}, "other": {"anies": [{"name": "referenceToUnitGroupDataSet", "value": {"shortDescription": [{"value": "CTUh", "lang": "de"}], "type": "unit group data set", "refObjectId": "d4c9523e-2d7e-49fd-8469-998f547d3a70", "uri": "../unitgroups/d4c9523e-2d7e-49fd-8469-998f547d3a70.xml"}}, {"module": "A1-A3"}, {"module": "A4"}, {"module": "A5"}, {"module": "C2"}, {"module": "C4"}, {"module": "D"}]}}, {"referenceToLCIAMethodDataSet": {"shortDescription": [{"value": "Toxizitätsvergleichseinheit für Menschen (nicht krebserregend) (HTP-nc)", "lang": "de"}, {"value": "Comparative toxic unit for humans (noncarcinogenic) (HTP-nc)", "lang": "en"}], "type": "LCIA method data set", "refObjectId": "3af763a5-b7a1-48c9-9cee-1f223481fcef", "uri": "../lciamethods/3af763a5-b7a1-48c9-9cee-1f223481fcef.xml"}, "other": {"anies": [{"name": "referenceToUnitGroupDataSet", "value": {"shortDescription": [{"value": "CTUh", "lang": "de"}], "type": "unit group data set", "refObjectId": "d4c9523e-2d7e-49fd-8469-998f547d3a70", "uri": "../unitgroups/d4c9523e-2d7e-49fd-8469-998f547d3a70.xml"}}, {"module": "A1-A3"}, {"module": "A4"}, {"module": "A5"}, {"module": "C2"}, {"module": "C4"}, {"module": "D"}]}}, {"referenceToLCIAMethodDataSet": {"shortDescription": [{"value": "Bodenqualitätsindex (SQP)", "lang": "de"}, {"value": "Soil quality index (SQP)", "lang": "en"}], "type": "LCIA method data set", "refObjectId": "b2ad6890-c78d-11e6-9d9d-cec0c932ce01", "uri": "../lciamethods/b2ad6890-c78d-11e6-9d9d-cec0c932ce01.xml"}, "other": {"anies": [{"name": "referenceToUnitGroupDataSet", "value": {"shortDescription": [{"value": "SQP", "lang": "de"}], "type": "unit group data set", "refObjectId": "f130951c-e67f-4f7f-8dd4-665de3974e18", "uri": "../unitgroups/f130951c-e67f-4f7f-8dd4-665de3974e18.xml"}}, {"module": "A1-A3"}, {"module": "A4"}, {"module": "A5"}, {"module": "C2"}, {"module": "C4"}, {"module": "D"}]}}]}, "otherAttributes": {"{http://www.indata.network/EPD/2019}epd-version": "1.2"}, "version": "1.1", "locations": "../ILCDLocations.xml"}