{"processInformation": {"dataSetInformation": {"UUID": "f8044564-a448-455e-9c9c-476b7a7c69e4", "name": {"baseName": [{"value": "MeisterDesign.pro, total weight 3,4 kg/m²", "lang": "en"}, {"value": "Elastischer Polyurethan Bodenbelag, maximales Gesamtgewicht 3,4 kg/m²", "lang": "de"}], "functionalUnitFlowProperties": [{"lang": "en"}]}, "classificationInformation": {"classification": [{"class": [{"value": "Kunststoffe", "level": 0, "classId": "6"}, {"value": "Bodenbeläge", "level": 1, "classId": "6.2"}, {"value": "Mehrschichtig modulare Bodenbeläge", "level": 2, "classId": "6.2.06"}], "name": "OEKOBAU.DAT"}, {"class": [{"value": "02 Building products", "level": 0}, {"value": "Floor coverings", "level": 1}, {"value": "Floor coverings", "level": 2}], "name": "IBUCategories"}]}, "generalComment": [{"value": "The resilient floor covering based on polyurethane is produced with the reactive component castor oil as renewable raw material and with natural inorganic filler. Products are available in many different decors and textures and it is offered as rolls or as planks. The declaration applies to a product with a maximum total weight of 3,4 kg/m.", "lang": "en"}, {"value": "Der elastische Bodenbelag auf Basis von Polyurethan wird mit der reaktiven Komponente Rizinusöl als nachwachsendem Rohstoff und mit natürlichem anorganischem Füllstoff hergestellt. Die Produkte sind in vielen verschiedenen Dekoren und Texturen erhältlich und werden als Rollen oder Dielen angeboten. Die Deklaration gilt für ein Produkt mit einem maximalen Gesamtgewicht von 3,4 kg/m².", "lang": "de"}], "other": {"anies": [{"scenario": [{"description": [{"value": "Deponie", "lang": "en"}, {"value": "Deponie", "lang": "de"}], "name": "S1", "default": true}, {"description": [{"value": "Verbrennung", "lang": "en"}, {"value": "Verbrennung", "lang": "de"}], "name": "S2"}, {"description": [{"value": "Zementwerk", "lang": "en"}, {"value": "Zementwerk", "lang": "de"}], "name": "S3"}]}]}}, "quantitativeReference": {"referenceToReferenceFlow": [0]}, "time": {"referenceYear": 2024, "dataSetValidUntil": 2029, "other": {"anies": [{"name": "publicationDateOfEPD", "value": 1712188800000}]}}, "geography": {"locationOfOperationSupplyOrProduction": {"location": "RER"}}, "technology": {"technologyDescriptionAndIncludedProcesses": [{"value": "\"PURLINE\" - resilient floor covering based on polyurethane is produced with the reactive component castor oil as renewable raw material and with natural inorganic filler.", "lang": "en"}, {"value": "Polyurethan Bodenbelag zum Kleben hergestellt im Rakelverfahren mit einem Anteil an erneuerbarem Material in der Hauptkomponente PU \nTechnische Daten: \nProdukt Form: Planken oder Rollen\nArt der Herstellung: Rakelverfahren\nGesamtgewicht: max. 3400 g/m²  \nDeklarierte Einheit: \nDeklarierte Einheit\nDie angegebene Einheit bezieht sich auf 1 m²  produzierten elastischen Bodenbelag. Der Output von Modul A5 \"Montage\" ist 1 m² verlegter textiler Bodenbelag. Die Rohdichte beträgt 1700 kg/m^3.", "lang": "de"}], "technologicalApplicability": [{"value": "According to the use class as defined in ISO 10874 the product can be used\n- in domestic areas, classified as use class 23,\n- in commercial areas, classified as use class 33", "lang": "en"}, {"value": "Gemäß der in ISO 10874 definierten Verwendungsklasse kann das Produkt verwendet werden - im häuslichen Bereich, klassifiziert als Verwendungsklasse 23, - im gewerblichen Bereich, klassifiziert als Verwendungsklasse 33 und 43", "lang": "de"}]}}, "modellingAndValidation": {"LCIMethodAndAllocation": {"typeOfDataSet": "EPD", "referenceToLCAMethodDetails": [{"shortDescription": [{"value": "Floor coverings.pdf", "lang": "en"}], "type": "source data set", "refObjectId": "f9f0d656-1866-4703-afbd-4e19aa3220cb"}], "other": {"anies": [{"name": "subType", "value": "specific dataset"}]}}, "dataSourcesTreatmentAndRepresentativeness": {"referenceToDataSource": [{"shortDescription": [{"value": "GaBi Database (all versions)", "lang": "en"}], "type": "source data set", "refObjectId": "28d74cc0-db8b-4d7e-bc44-5f6d56ce0c4a"}, {"shortDescription": [{"value": "Sphera MLC (fka GaBi) CUP 2023.01", "lang": "en"}], "type": "source data set", "refObjectId": "6bcd5bfa-3623-48ab-a52b-6d5be8db82ed"}], "useAdviceForDataSet": [{"value": "Scope: \nThe manufacturer declaration applies to products with a maximum total weight of 3,4 kg/m.\nThe product is available as planks. It is manufactured in Germany. \nSystem boundary: \nType of EPD: Cradle-to-grave\n\nSystem boundaries of modules A, B, C, D:\n\nA1-A3 Production:\nEnergy supply and production of the basic material, auxiliary material, transport of the material to the manufacturing site, emissions, waste water treatment, packaging material and waste processing up to the landfill disposal of residual waste (except radioactive waste). Benefits for generated electricity and steam due to the incineration of production waste are aggregated.\n\nA4 Transport:\nTransport of the packed floor covering from factory gate to the place of installation.\n\nA5 Installation:\nInstallation of the floor covering, processing of installation waste and packaging waste up to the landfill disposal of residual waste (except radioactive waste), the production of the amount of floor covering that occurs as installation waste including its transport to the place of installation. Generated electricity and steam due to the incineration of waste are listed in the result table as exported energy. Preparing of the floor and adhesives are beyond the system boundaries and not taken into account.\n\nB1 Use:\nIndoor emissions during the use stage. After the first year, no product-related volatile organic compoun (VOC) emissions are relevant due to the VOC decay curves of the product.\n\nB2 Maintenance:\nCleaning of the floor covering for a period of 1 year:\nWet cleaning – water consumption, production of the cleaning agent, waste water treatment.\nThe declared values in this module have to be multiplied by the assumed service life of the floor covering in the building in question (see annexe, chapter General information on use stage).\n\nB3 - B7:\nThe modules are not relevant and therefore not declared.\n\nC1 De-construction:\nEnergy consumption of the de-construction machine.\n\nC2 Transport:\nTransport of the floor covering waste to a landfill or to the municipal waste incineration plant (MWI).\n\nC3 Waste processing:\nC3-1: Landfill disposal needs no waste processing.\nC3-2: Impact from waste incineration (plant with R1 > 0.6), generated electricity and steam are listed in the result table as exported energy.\nC3-3: Collection of the carpet waste for recovery in the cement industry, waste processing (granulating), transport to the cement plant, emissions from the incineration.\n\nC4 Disposal:\nC4-1: Impact from landfill disposal,\nC4-2: The carpet waste leaves the system in module C3-2,\nC4-3: The pre-processed carpet waste leaves the system in\nmodule C3-3\n\nD Recycling potential:\nCalculated benefits result from materials exclusive secondary materials (net materials).\nD-A5: Benefits for generated energy due to incineration of packaging and installation waste (incineration plant with R1 > 0.6),\nD-1: Benefits for generated energy due to landfill disposal of carpet waste at the end of life,\nD-2: Benefits for generated energy due to incineration of carpet waste at the end-of-life (incineration plant with R1 > 0.6),\nD-3: Benefits for saved fossil energy and saved inorganic material due to recovery of the carpet in a cement plant.(incineration plant with R1 > 0.6),", "lang": "en"}, {"value": "Gültigkeitsbereich: \nDie Herstellererklärung gilt für Produkte mit einem maximalen Gesamtgewicht von 3,4 kg/m². Das Produkt ist als Rollen oder Bohlen erhältlich. Es wird am Standort der Windmöller GmbH in Detmold, Deutschland, hergestellt. Der Zuschnitt der Bohlen erfolgt am Standort der Windmöller GmbH in Augustdorf, Deutschland. \nSystemgrenze: \nArt der EPD: Cradle-to-Grave Systemgrenzen der Module A, B, C, D: A1-A3 Produktion: Energieversorgung und Produktion des Grundmaterials, Hilfsstoffe, Transport des Materials zum Herstellungsort, Emissionen, Abwasseraufbereitung, Verpackungsmaterial und Abfallverarbeitung bis hin zur Deponierung von Restmüll (außer radioaktivem Abfall). Leistungen für erzeugten Strom und Dampf aufgrund der Verbrennung von Produktionsabfällen werden zusammengefasst. A4 Transport: Transport des verpackten Bodenbelags vom Werkstor zum Verlegeort. A5 Verlegung: Verlegung des Bodenbelags, Aufbereitung von Verlegeabfällen und Verpackungsabfällen bis zur Deponierung von Restmüll (außer radioaktiven Abfällen), die Herstellung der als Verlegeabfall anfallenden Bodenbelagsmenge einschließlich deren Transport zum Verlegeort. Der durch die Verbrennung von Abfällen erzeugte Strom und Dampf wird in der Ergebnistabelle als exportierte Energie aufgeführt. Die Vorbereitung des Bodens und der Klebstoffe liegen außerhalb der Systemgrenzen und werden nicht berücksichtigt. B1 Nutzung: Emissionen in Innenräumen während der Nutzungsphase. Nach dem ersten Jahr sind aufgrund der VOC-Abklingkurven des Produkts keine produktbezogenen Emissionen flüchtiger organischer Verbindungen (VOC) mehr relevant. B2 Wartung: Reinigung des Bodenbelags für einen Zeitraum von 1 Jahr: Staubsaugen - Stromzufuhr Nassreinigung - Wasserverbrauch, Herstellung des Reinigungsmittels, Abwasseraufbereitung.\nDie deklarierten Werte in diesem Modul müssen mit der angenommenen Lebensdauer des Bodenbelags in dem betreffenden Gebäude multipliziert werden (siehe Anhang, Kapitel 'Allgemeine Informationen zur Nutzungsphase'). B3 - B7: Die Module sind nicht relevant und werden daher nicht deklariert. C1 Rückbau: Energieverbrauch der Rückbaumaschine. C2 Transport: Transport der Bodenbelagsabfälle zu einer Deponie oder zur kommunalen Müllverbrennungsanlage (KVA). C3 Abfallverarbeitung: C3-1: Die Deponierung erfordert keine Abfallverarbeitung. \nC3-2: Auswirkungen der Abfallverbrennung (Anlage mit R1>0,6), erzeugter Strom und Dampf werden in der Ergebnistabelle als exportierte Energie aufgeführt. C4 Entsorgung C4-1: Auswirkungen der Deponieentsorgung, C4-2: Die Bodenbelagsabfälle verlassen das System in Modul C3-2, D Recyclingpotenzial: D-A5: Nutzen für die erzeugte Energie aufgrund der Verbrennung von Verpackungs- und Installationsabfällen (Verbrennungsanlage mit R1 > 0.6), D-1: Nutzen für die erzeugte Energie aufgrund der Deponierung von Bodenbelagsabfällen am Ende des Lebenszyklus, D-2: Nutzen für die erzeugte Energie aufgrund der Verbrennung von Bodenbelagsabfällen am Ende des Lebenszyklus (Verbrennungsanlage mit R1 > 0,6),", "lang": "de"}], "other": {"anies": [{"name": "referenceToOriginalEPD", "value": {"shortDescription": {"value": "MeisterDesign.pro, total weight 3,4 kg/m².pdf", "defaultValue": "MeisterDesign.pro, total weight 3,4 kg/m².pdf", "lstrings": [{"lang": "en", "value": "MeisterDesign.pro, total weight 3,4 kg/m².pdf"}]}, "type": "source data set", "uuid": {"uuid": "64d7543b-29fa-429d-85a3-ac5b5bbdadee"}, "refObjectId": "64d7543b-29fa-429d-85a3-ac5b5bbdadee", "resourceURLs": ["https://oekobaudat.de/OEKOBAU.DAT/resource/sources/64d7543b-29fa-429d-85a3-ac5b5bbdadee/MeisterDesign.pro_total_weight_3_4_kgm_22901.pdf?version=00.02.000"]}}]}}, "validation": {"review": [{"referenceToNameOfReviewerAndInstitution": [{"shortDescription": [{"value": "Institut Bauen und Umwelt e. V.", "lang": "en"}], "type": "contact data set", "refObjectId": "d111dbec-b024-4be5-86c5-752d6eb2cf95", "uri": "../contacts/d111dbec-b024-4be5-86c5-752d6eb2cf95.xml"}], "type": "Accredited third party review"}]}, "complianceDeclarations": {"compliance": [{"referenceToComplianceSystem": {"shortDescription": [{"value": "EN 15804+A2 (EF 3.1)", "lang": "en"}], "type": "source data set", "refObjectId": "d4aa3ec7-b1d7-4a4a-a6cb-37af88dcc902", "uri": "../sources/d4aa3ec7-b1d7-4a4a-a6cb-37af88dcc902.xml"}}, {"referenceToComplianceSystem": {"shortDescription": [{"value": "ISO 14025", "lang": "en"}], "type": "source data set", "refObjectId": "4f2eb655-6e44-4874-a95a-e28f5442cd4d", "uri": "../sources/4f2eb655-6e44-4874-a95a-e28f5442cd4d.xml"}}]}}, "administrativeInformation": {"commissionerAndGoal": {"referenceToCommissioner": [{"shortDescription": [{"value": "MeisterWerke Schulte GmbH", "lang": "en"}], "type": "contact data set", "refObjectId": "79282f4b-72bc-4c40-a60e-5e7ac802336a", "uri": "../contacts/79282f4b-72bc-4c40-a60e-5e7ac802336a.xml"}]}, "dataGenerator": {"referenceToPersonOrEntityGeneratingTheDataSet": [{"shortDescription": [{"value": "Gemeinschaft umweltfreundlicher Teppichboden (GUT) e.V.", "lang": "en"}], "type": "contact data set", "refObjectId": "1e593d93-ef5b-4ddc-9b55-f58cf8960f3e", "uri": "../contacts/1e593d93-ef5b-4ddc-9b55-f58cf8960f3e.xml"}]}, "dataEntryBy": {"timeStamp": 1712188800000, "referenceToDataSetFormat": [{"shortDescription": [{"value": "ILCD Format", "lang": "en"}], "type": "source data set", "refObjectId": "a97a0155-0234-4b87-b4ce-a45da52f2a40", "uri": "../sources/a97a0155-0234-4b87-b4ce-a45da52f2a40.xml"}, {"shortDescription": [{"value": "EPD-Datenformaterweiterungen v1.2", "lang": "de"}, {"value": "EPD Data Format Extensions v1.2", "lang": "en"}], "type": "source data set", "refObjectId": "a29449fd-aa2f-4de8-b5d7-4b06b43c6fde", "uri": "../sources/a29449fd-aa2f-4de8-b5d7-4b06b43c6fde.xml"}]}, "publicationAndOwnership": {"dataSetVersion": "00.03.100", "referenceToRegistrationAuthority": {"shortDescription": [{"value": "Institut Bauen und Umwelt e. V.", "lang": "en"}], "type": "contact data set", "refObjectId": "d111dbec-b024-4be5-86c5-752d6eb2cf95", "uri": "../contacts/d111dbec-b024-4be5-86c5-752d6eb2cf95.xml"}, "registrationNumber": "EPD-MWS-20240569-CBA2-EN", "referenceToOwnershipOfDataSet": {"shortDescription": [{"value": "MeisterWerke Schulte GmbH", "lang": "en"}], "type": "contact data set", "refObjectId": "79282f4b-72bc-4c40-a60e-5e7ac802336a", "uri": "../contacts/79282f4b-72bc-4c40-a60e-5e7ac802336a.xml"}, "copyright": true, "licenseType": "Free of charge for all users and uses", "accessRestrictions": [{"value": "None", "lang": "en"}], "other": {"anies": [{"name": "referenceToPublisher", "value": {"shortDescription": [{"value": "Institut Bauen und Umwelt e. V.", "lang": "en"}], "type": "contact data set", "refObjectId": "d111dbec-b024-4be5-86c5-752d6eb2cf95", "uri": "../contacts/d111dbec-b024-4be5-86c5-752d6eb2cf95.xml"}}]}}}, "exchanges": {"exchange": [{"dataSetInternalID": 0, "referenceToFlowDataSet": {"shortDescription": [{"value": "MeisterDesign.pro, total weight 3,4 kg/m² (Elastischer PU Bodenbelag zum Kleben)", "lang": "en"}], "type": "flow data set", "refObjectId": "d2a7404e-3c7c-b13f-71a6-13d79ff9f58a", "uri": "../flows/d2a7404e-3c7c-b13f-71a6-13d79ff9f58a.xml"}, "meanAmount": 1.0, "referencesToDataSource": {}, "referenceFlow": true, "resolvedFlowVersion": "00.03.000", "resultingflowAmount": 1.0, "flowProperties": [{"name": [{"lang": "de", "value": "Fläche"}, {"lang": "en", "value": "Area"}], "uuid": "93a60a56-a3c8-19da-a746-0800200c9a66", "referenceFlowProperty": true, "meanValue": 1.0, "referenceUnit": "qm", "unitGroupUUID": "c20a03d7-bd90-4569-bc94-66cfd364dfc8"}], "materialProperties": [{"name": "grammage", "value": "3.4", "unit": "kg/m^2", "unitDescription": "kilograms per square meter"}, {"name": "layer thickness", "value": "0.002", "unit": "m", "unitDescription": "meters"}, {"name": "gross density", "value": "1700.0", "unit": "kg/m^3", "unitDescription": "kilograms per cubic metre"}], "typeOfFlow": "Product flow", "classification": {"classHierarchy": "Kunststoffe / Bodenbeläge / Mehrschichtig modulare Bodenbeläge", "name": "OEKOBAU.DAT"}}, {"dataSetInternalID": 1, "referenceToFlowDataSet": {"shortDescription": [{"value": "Renewable primary energy as energy carrier (PERE)", "lang": "en"}, {"value": "Erneuerbare Primärenergie als Energieträger (PERE)", "lang": "de"}], "type": "flow data set", "refObjectId": "20f32be5-0398-4288-9b6d-accddd195317", "uri": "../flows/20f32be5-0398-4288-9b6d-accddd195317.xml"}, "exchange direction": "INPUT", "other": {"anies": [{"name": "referenceToUnitGroupDataSet", "value": {"shortDescription": [{"value": "MJ", "lang": "en"}], "type": "unit group data set", "refObjectId": "93a60a57-a3c8-11da-a746-0800200c9a66", "uri": "../unitgroups/93a60a57-a3c8-11da-a746-0800200c9a66.xml"}}, {"value": "16.167", "module": "A1-A3"}, {"value": "0.1946", "module": "A4"}, {"value": "1.21779", "module": "A5"}, {"value": "0", "module": "B1"}, {"value": "9.146", "module": "B2"}, {"value": "0", "module": "C1"}, {"value": "0.01356", "module": "C2"}, {"module": "C3"}, {"module": "C3", "scenario": "S1"}, {"value": "21.8123", "module": "C3", "scenario": "S2"}, {"value": "22.0379", "module": "C3", "scenario": "S3"}, {"module": "C4"}, {"value": "0.315", "module": "C4", "scenario": "S1"}, {"module": "C4", "scenario": "S2"}, {"module": "C4", "scenario": "S3"}, {"value": "-0.1269", "module": "D"}, {"value": "0", "module": "D", "scenario": "S1"}, {"value": "-4.229", "module": "D", "scenario": "S2"}, {"value": "-0.3866", "module": "D", "scenario": "S3"}]}, "resolvedFlowVersion": "38.00.000", "flowProperties": [], "typeOfFlow": "Other flow", "classification": {"classHierarchy": "Quantities", "name": "GaBiCategories"}}, {"dataSetInternalID": 2, "referenceToFlowDataSet": {"shortDescription": [{"value": "Renewable primary energy resources as material utilization (PERM)", "lang": "en"}, {"value": "Erneuerbare Primärenergie zur stofflichen Nutzung (PERM)", "lang": "de"}], "type": "flow data set", "refObjectId": "fb3ec0de-548d-4508-aea5-00b73bf6f702", "uri": "../flows/fb3ec0de-548d-4508-aea5-00b73bf6f702.xml"}, "exchange direction": "INPUT", "other": {"anies": [{"name": "referenceToUnitGroupDataSet", "value": {"shortDescription": [{"value": "MJ", "lang": "en"}], "type": "unit group data set", "refObjectId": "93a60a57-a3c8-11da-a746-0800200c9a66", "uri": "../unitgroups/93a60a57-a3c8-11da-a746-0800200c9a66.xml"}}, {"value": "21.493", "module": "A1-A3"}, {"value": "0", "module": "A4"}, {"value": "-0.07", "module": "A5"}, {"value": "0", "module": "B1"}, {"value": "0", "module": "B2"}, {"value": "0", "module": "C1"}, {"value": "0", "module": "C2"}, {"module": "C3"}, {"module": "C3", "scenario": "S1"}, {"value": "-21.423", "module": "C3", "scenario": "S2"}, {"value": "-21.423", "module": "C3", "scenario": "S3"}, {"module": "C4"}, {"value": "0", "module": "C4", "scenario": "S1"}, {"module": "C4", "scenario": "S2"}, {"module": "C4", "scenario": "S3"}, {"value": "0", "module": "D"}, {"value": "0", "module": "D", "scenario": "S1"}, {"value": "0", "module": "D", "scenario": "S2"}, {"value": "0", "module": "D", "scenario": "S3"}]}, "resolvedFlowVersion": "38.00.000", "flowProperties": [], "typeOfFlow": "Other flow", "classification": {"classHierarchy": "Quantities", "name": "GaBiCategories"}}, {"dataSetInternalID": 3, "referenceToFlowDataSet": {"shortDescription": [{"value": "Total use of renewable primary energy resources (PERT)", "lang": "en"}, {"value": "Total erneuerbare Primärenergie (PERT)", "lang": "de"}], "type": "flow data set", "refObjectId": "53f97275-fa8a-4cdd-9024-65936002acd0", "uri": "../flows/53f97275-fa8a-4cdd-9024-65936002acd0.xml"}, "exchange direction": "INPUT", "other": {"anies": [{"name": "referenceToUnitGroupDataSet", "value": {"shortDescription": [{"value": "MJ", "lang": "en"}], "type": "unit group data set", "refObjectId": "93a60a57-a3c8-11da-a746-0800200c9a66", "uri": "../unitgroups/93a60a57-a3c8-11da-a746-0800200c9a66.xml"}}, {"value": "37.66", "module": "A1-A3"}, {"value": "0.1946", "module": "A4"}, {"value": "1.14779", "module": "A5"}, {"value": "0", "module": "B1"}, {"value": "9.146", "module": "B2"}, {"value": "0", "module": "C1"}, {"value": "0.01356", "module": "C2"}, {"module": "C3"}, {"module": "C3", "scenario": "S1"}, {"value": "0.3893", "module": "C3", "scenario": "S2"}, {"value": "0.6149", "module": "C3", "scenario": "S3"}, {"module": "C4"}, {"value": "0.315", "module": "C4", "scenario": "S1"}, {"module": "C4", "scenario": "S2"}, {"module": "C4", "scenario": "S3"}, {"value": "-0.1269", "module": "D"}, {"value": "0", "module": "D", "scenario": "S1"}, {"value": "-4.229", "module": "D", "scenario": "S2"}, {"value": "-0.3866", "module": "D", "scenario": "S3"}]}, "resolvedFlowVersion": "38.00.000", "flowProperties": [], "typeOfFlow": "Other flow", "classification": {"classHierarchy": "Quantities / Environmental quantities / EPD EN 15804 / LCI indicators", "name": "GaBiCategories"}}, {"dataSetInternalID": 4, "referenceToFlowDataSet": {"shortDescription": [{"value": "Non renewable primary energy as energy carrier (PENRE)", "lang": "en"}, {"value": "Nicht-erneuerbare Primärenergie als Energieträger (PENRE)", "lang": "de"}], "type": "flow data set", "refObjectId": "ac857178-2b45-46ec-892a-a9a4332f0372", "uri": "../flows/ac857178-2b45-46ec-892a-a9a4332f0372.xml"}, "exchange direction": "INPUT", "other": {"anies": [{"name": "referenceToUnitGroupDataSet", "value": {"shortDescription": [{"value": "MJ", "lang": "en"}], "type": "unit group data set", "refObjectId": "93a60a57-a3c8-11da-a746-0800200c9a66", "uri": "../unitgroups/93a60a57-a3c8-11da-a746-0800200c9a66.xml"}}, {"value": "61.446", "module": "A1-A3"}, {"value": "3.433", "module": "A4"}, {"value": "2.7526", "module": "A5"}, {"value": "0", "module": "B1"}, {"value": "13.84", "module": "B2"}, {"value": "0", "module": "C1"}, {"value": "0.192", "module": "C2"}, {"module": "C3"}, {"module": "C3", "scenario": "S1"}, {"value": "18.004", "module": "C3", "scenario": "S2"}, {"value": "18.804", "module": "C3", "scenario": "S3"}, {"module": "C4"}, {"value": "3.492", "module": "C4", "scenario": "S1"}, {"module": "C4", "scenario": "S2"}, {"module": "C4", "scenario": "S3"}, {"value": "-0.4482", "module": "D"}, {"value": "0", "module": "D", "scenario": "S1"}, {"value": "-14.94", "module": "D", "scenario": "S2"}, {"value": "-40.37", "module": "D", "scenario": "S3"}]}, "resolvedFlowVersion": "38.00.000", "flowProperties": [], "typeOfFlow": "Other flow", "classification": {"classHierarchy": "Quantities", "name": "GaBiCategories"}}, {"dataSetInternalID": 5, "referenceToFlowDataSet": {"shortDescription": [{"value": "Non renewable primary energy as material utilization (PENRM)", "lang": "en"}, {"value": "Nicht-erneuerbare Primärenergie zur stofflichen Nutzung (PENRM)", "lang": "de"}], "type": "flow data set", "refObjectId": "1421caa0-679d-4bf4-b282-0eb850ccae27", "uri": "../flows/1421caa0-679d-4bf4-b282-0eb850ccae27.xml"}, "exchange direction": "INPUT", "other": {"anies": [{"name": "referenceToUnitGroupDataSet", "value": {"shortDescription": [{"value": "MJ", "lang": "en"}], "type": "unit group data set", "refObjectId": "93a60a57-a3c8-11da-a746-0800200c9a66", "uri": "../unitgroups/93a60a57-a3c8-11da-a746-0800200c9a66.xml"}}, {"value": "16.154", "module": "A1-A3"}, {"value": "0", "module": "A4"}, {"value": "-0.252", "module": "A5"}, {"value": "0", "module": "B1"}, {"value": "0", "module": "B2"}, {"value": "0", "module": "C1"}, {"value": "0", "module": "C2"}, {"module": "C3"}, {"module": "C3", "scenario": "S1"}, {"value": "-15.902", "module": "C3", "scenario": "S2"}, {"value": "-15.902", "module": "C3", "scenario": "S3"}, {"module": "C4"}, {"value": "0", "module": "C4", "scenario": "S1"}, {"module": "C4", "scenario": "S2"}, {"module": "C4", "scenario": "S3"}, {"value": "0", "module": "D"}, {"value": "0", "module": "D", "scenario": "S1"}, {"value": "0", "module": "D", "scenario": "S2"}, {"value": "0", "module": "D", "scenario": "S3"}]}, "resolvedFlowVersion": "38.00.000", "flowProperties": [], "typeOfFlow": "Other flow", "classification": {"classHierarchy": "Quantities", "name": "GaBiCategories"}}, {"dataSetInternalID": 6, "referenceToFlowDataSet": {"shortDescription": [{"value": "Total use of non renewable primary energy resources (PENRT)", "lang": "en"}, {"value": "Total nicht erneuerbare Primärenergie (PENRT)", "lang": "de"}], "type": "flow data set", "refObjectId": "06159210-646b-4c8d-8583-da9b3b95a6c1", "uri": "../flows/06159210-646b-4c8d-8583-da9b3b95a6c1.xml"}, "exchange direction": "INPUT", "other": {"anies": [{"name": "referenceToUnitGroupDataSet", "value": {"shortDescription": [{"value": "MJ", "lang": "en"}], "type": "unit group data set", "refObjectId": "93a60a57-a3c8-11da-a746-0800200c9a66", "uri": "../unitgroups/93a60a57-a3c8-11da-a746-0800200c9a66.xml"}}, {"value": "77.6", "module": "A1-A3"}, {"value": "3.433", "module": "A4"}, {"value": "2.5006", "module": "A5"}, {"value": "0", "module": "B1"}, {"value": "13.84", "module": "B2"}, {"value": "0", "module": "C1"}, {"value": "0.192", "module": "C2"}, {"module": "C3"}, {"module": "C3", "scenario": "S1"}, {"value": "2.102", "module": "C3", "scenario": "S2"}, {"value": "2.902", "module": "C3", "scenario": "S3"}, {"module": "C4"}, {"value": "3.492", "module": "C4", "scenario": "S1"}, {"module": "C4", "scenario": "S2"}, {"module": "C4", "scenario": "S3"}, {"value": "-0.4482", "module": "D"}, {"value": "0", "module": "D", "scenario": "S1"}, {"value": "-14.94", "module": "D", "scenario": "S2"}, {"value": "-40.37", "module": "D", "scenario": "S3"}]}, "resolvedFlowVersion": "38.00.000", "flowProperties": [], "typeOfFlow": "Other flow", "classification": {"classHierarchy": "Quantities / Environmental quantities / EPD EN 15804 / LCI indicators", "name": "GaBiCategories"}}, {"dataSetInternalID": 7, "referenceToFlowDataSet": {"shortDescription": [{"value": "Use of secondary material (SM)", "lang": "en"}, {"value": "Einsatz von Sekundärstoffen (SM)", "lang": "de"}], "type": "flow data set", "refObjectId": "c6a1f35f-2d09-4f54-8dfb-97e502e1ce92", "uri": "../flows/c6a1f35f-2d09-4f54-8dfb-97e502e1ce92.xml"}, "exchange direction": "INPUT", "other": {"anies": [{"name": "referenceToUnitGroupDataSet", "value": {"shortDescription": [{"value": "kg", "lang": "en"}], "type": "unit group data set", "refObjectId": "ad38d542-3fe9-439d-9b95-2f5f7752acaf", "uri": "../unitgroups/ad38d542-3fe9-439d-9b95-2f5f7752acaf.xml"}}, {"value": "0.02148", "module": "A1-A3"}, {"value": "0", "module": "A4"}, {"value": "0.0006444", "module": "A5"}, {"value": "0", "module": "B1"}, {"value": "0", "module": "B2"}, {"value": "0", "module": "C1"}, {"value": "0", "module": "C2"}, {"module": "C3"}, {"module": "C3", "scenario": "S1"}, {"value": "0", "module": "C3", "scenario": "S2"}, {"value": "0", "module": "C3", "scenario": "S3"}, {"module": "C4"}, {"value": "0", "module": "C4", "scenario": "S1"}, {"module": "C4", "scenario": "S2"}, {"module": "C4", "scenario": "S3"}, {"value": "0", "module": "D"}, {"value": "0", "module": "D", "scenario": "S1"}, {"value": "0", "module": "D", "scenario": "S2"}, {"value": "1.29", "module": "D", "scenario": "S3"}]}, "resolvedFlowVersion": "38.00.000", "flowProperties": [], "typeOfFlow": "Other flow", "classification": {"classHierarchy": "Quantities / Environmental quantities / EPD EN 15804 / LCI indicators", "name": "GaBiCategories"}}, {"dataSetInternalID": 8, "referenceToFlowDataSet": {"shortDescription": [{"value": "Use of renewable secondary fuels (RSF)", "lang": "en"}, {"value": "Erneuerbare Sekundärbrennstoffe (RSF)", "lang": "de"}], "type": "flow data set", "refObjectId": "64333088-a55f-4aa2-9a31-c10b07816787", "uri": "../flows/64333088-a55f-4aa2-9a31-c10b07816787.xml"}, "exchange direction": "INPUT", "other": {"anies": [{"name": "referenceToUnitGroupDataSet", "value": {"shortDescription": [{"value": "MJ", "lang": "en"}], "type": "unit group data set", "refObjectId": "93a60a57-a3c8-11da-a746-0800200c9a66", "uri": "../unitgroups/93a60a57-a3c8-11da-a746-0800200c9a66.xml"}}, {"value": "0", "module": "A1-A3"}, {"value": "0", "module": "A4"}, {"value": "0", "module": "A5"}, {"value": "0", "module": "B1"}, {"value": "0", "module": "B2"}, {"value": "0", "module": "C1"}, {"value": "0", "module": "C2"}, {"module": "C3"}, {"module": "C3", "scenario": "S1"}, {"value": "0", "module": "C3", "scenario": "S2"}, {"value": "0", "module": "C3", "scenario": "S3"}, {"module": "C4"}, {"value": "0", "module": "C4", "scenario": "S1"}, {"module": "C4", "scenario": "S2"}, {"module": "C4", "scenario": "S3"}, {"value": "0", "module": "D"}, {"value": "0", "module": "D", "scenario": "S1"}, {"value": "0", "module": "D", "scenario": "S2"}, {"value": "0", "module": "D", "scenario": "S3"}]}, "resolvedFlowVersion": "38.00.000", "flowProperties": [], "typeOfFlow": "Other flow", "classification": {"classHierarchy": "Quantities / Environmental quantities / EPD EN 15804 / LCI indicators", "name": "GaBiCategories"}}, {"dataSetInternalID": 9, "referenceToFlowDataSet": {"shortDescription": [{"value": "Use of non renewable secondary fuels (NRSF)", "lang": "en"}, {"value": "Nicht erneuerbare Sekundärbrennstoffe (NRSF)", "lang": "de"}], "type": "flow data set", "refObjectId": "89def144-d39a-4287-b86f-efde453ddcb2", "uri": "../flows/89def144-d39a-4287-b86f-efde453ddcb2.xml"}, "exchange direction": "INPUT", "other": {"anies": [{"name": "referenceToUnitGroupDataSet", "value": {"shortDescription": [{"value": "MJ", "lang": "en"}], "type": "unit group data set", "refObjectId": "93a60a57-a3c8-11da-a746-0800200c9a66", "uri": "../unitgroups/93a60a57-a3c8-11da-a746-0800200c9a66.xml"}}, {"value": "0", "module": "A1-A3"}, {"value": "0", "module": "A4"}, {"value": "0", "module": "A5"}, {"value": "0", "module": "B1"}, {"value": "0", "module": "B2"}, {"value": "0", "module": "C1"}, {"value": "0", "module": "C2"}, {"module": "C3"}, {"module": "C3", "scenario": "S1"}, {"value": "0", "module": "C3", "scenario": "S2"}, {"value": "0", "module": "C3", "scenario": "S3"}, {"module": "C4"}, {"value": "0", "module": "C4", "scenario": "S1"}, {"module": "C4", "scenario": "S2"}, {"module": "C4", "scenario": "S3"}, {"value": "0", "module": "D"}, {"value": "0", "module": "D", "scenario": "S1"}, {"value": "0", "module": "D", "scenario": "S2"}, {"value": "0", "module": "D", "scenario": "S3"}]}, "resolvedFlowVersion": "38.00.000", "flowProperties": [], "typeOfFlow": "Other flow", "classification": {"classHierarchy": "Quantities / Environmental quantities / EPD EN 15804 / LCI indicators", "name": "GaBiCategories"}}, {"dataSetInternalID": 10, "referenceToFlowDataSet": {"shortDescription": [{"value": "Use of net fresh water (FW)", "lang": "en"}, {"value": "Einsatz von Süßwasserressourcen (FW)", "lang": "de"}], "type": "flow data set", "refObjectId": "3cf952c8-f3a4-461d-8c96-96456ca62246", "uri": "../flows/3cf952c8-f3a4-461d-8c96-96456ca62246.xml"}, "exchange direction": "INPUT", "other": {"anies": [{"name": "referenceToUnitGroupDataSet", "value": {"shortDescription": [{"value": "m^3", "lang": "en"}], "type": "unit group data set", "refObjectId": "cd950537-0a98-4044-9ba7-9f9a68d0a504", "uri": "../unitgroups/cd950537-0a98-4044-9ba7-9f9a68d0a504.xml"}}, {"value": "2.35", "module": "A1-A3"}, {"value": "0.0002152", "module": "A4"}, {"value": "0.0708716", "module": "A5"}, {"value": "0", "module": "B1"}, {"value": "0.009777", "module": "B2"}, {"value": "0", "module": "C1"}, {"value": "1.494E-05", "module": "C2"}, {"module": "C3"}, {"module": "C3", "scenario": "S1"}, {"value": "0.01215", "module": "C3", "scenario": "S2"}, {"value": "0.01235", "module": "C3", "scenario": "S3"}, {"module": "C4"}, {"value": "3.444E-05", "module": "C4", "scenario": "S1"}, {"module": "C4", "scenario": "S2"}, {"module": "C4", "scenario": "S3"}, {"value": "-0.0001028", "module": "D"}, {"value": "0", "module": "D", "scenario": "S1"}, {"value": "-0.003427", "module": "D", "scenario": "S2"}, {"value": "-0.003508", "module": "D", "scenario": "S3"}]}, "resolvedFlowVersion": "38.00.000", "flowProperties": [], "typeOfFlow": "Other flow", "classification": {"classHierarchy": "Quantities / Environmental quantities / EPD EN 15804 / LCI indicators", "name": "GaBiCategories"}}, {"dataSetInternalID": 11, "referenceToFlowDataSet": {"shortDescription": [{"value": "Hazardous waste disposed (HWD)", "lang": "en"}, {"value": "Gefährlicher Abfall zur Deponie (HWD)", "lang": "de"}], "type": "flow data set", "refObjectId": "430f9e0f-59b2-46a0-8e0d-55e0e84948fc", "uri": "../flows/430f9e0f-59b2-46a0-8e0d-55e0e84948fc.xml"}, "exchange direction": "OUTPUT", "other": {"anies": [{"name": "referenceToUnitGroupDataSet", "value": {"shortDescription": [{"value": "kg", "lang": "en"}], "type": "unit group data set", "refObjectId": "ad38d542-3fe9-439d-9b95-2f5f7752acaf", "uri": "../unitgroups/ad38d542-3fe9-439d-9b95-2f5f7752acaf.xml"}}, {"value": "1.66E-08", "module": "A1-A3"}, {"value": "1.23E-11", "module": "A4"}, {"value": "5.0658E-10", "module": "A5"}, {"value": "0", "module": "B1"}, {"value": "0.000151", "module": "B2"}, {"value": "0", "module": "C1"}, {"value": "7.11E-13", "module": "C2"}, {"module": "C3"}, {"module": "C3", "scenario": "S1"}, {"value": "2.73E-10", "module": "C3", "scenario": "S2"}, {"value": "2.5E-10", "module": "C3", "scenario": "S3"}, {"module": "C4"}, {"value": "2.94E-10", "module": "C4", "scenario": "S1"}, {"module": "C4", "scenario": "S2"}, {"module": "C4", "scenario": "S3"}, {"value": "-2.54E-11", "module": "D"}, {"value": "0", "module": "D", "scenario": "S1"}, {"value": "-8.46E-10", "module": "D", "scenario": "S2"}, {"value": "-2.16E-12", "module": "D", "scenario": "S3"}]}, "resolvedFlowVersion": "38.00.000", "flowProperties": [], "typeOfFlow": "Other flow", "classification": {"classHierarchy": "Quantities / Environmental quantities / EPD EN 15804 / LCI indicators", "name": "GaBiCategories"}}, {"dataSetInternalID": 12, "referenceToFlowDataSet": {"shortDescription": [{"value": "Non hazardous waste disposed (NHWD)", "lang": "en"}, {"value": "Entsorgter nicht gefährlicher Abfall (NHWD)", "lang": "de"}], "type": "flow data set", "refObjectId": "b29ef66b-e286-4afa-949f-62f1a7b4d7fa", "uri": "../flows/b29ef66b-e286-4afa-949f-62f1a7b4d7fa.xml"}, "exchange direction": "OUTPUT", "other": {"anies": [{"name": "referenceToUnitGroupDataSet", "value": {"shortDescription": [{"value": "kg", "lang": "en"}], "type": "unit group data set", "refObjectId": "ad38d542-3fe9-439d-9b95-2f5f7752acaf", "uri": "../unitgroups/ad38d542-3fe9-439d-9b95-2f5f7752acaf.xml"}}, {"value": "0.179", "module": "A1-A3"}, {"value": "0.000457", "module": "A4"}, {"value": "0.03547", "module": "A5"}, {"value": "0", "module": "B1"}, {"value": "0.0355", "module": "B2"}, {"value": "0", "module": "C1"}, {"value": "2.77E-05", "module": "C2"}, {"module": "C3"}, {"module": "C3", "scenario": "S1"}, {"value": "1", "module": "C3", "scenario": "S2"}, {"value": "1", "module": "C3", "scenario": "S3"}, {"module": "C4"}, {"value": "3.39", "module": "C4", "scenario": "S1"}, {"module": "C4", "scenario": "S2"}, {"module": "C4", "scenario": "S3"}, {"value": "-0.000219", "module": "D"}, {"value": "0", "module": "D", "scenario": "S1"}, {"value": "-0.00729", "module": "D", "scenario": "S2"}, {"value": "-0.0216", "module": "D", "scenario": "S3"}]}, "resolvedFlowVersion": "38.00.000", "flowProperties": [], "typeOfFlow": "Other flow", "classification": {"classHierarchy": "Quantities / Environmental quantities / EPD EN 15804 / LCI indicators", "name": "GaBiCategories"}}, {"dataSetInternalID": 13, "referenceToFlowDataSet": {"shortDescription": [{"value": "Radioactive waste disposed (RWD)", "lang": "en"}, {"value": "Entsorgter radioaktiver Abfall (RWD)", "lang": "de"}], "type": "flow data set", "refObjectId": "3449546e-52ad-4b39-b809-9fb77cea8ff6", "uri": "../flows/3449546e-52ad-4b39-b809-9fb77cea8ff6.xml"}, "exchange direction": "OUTPUT", "other": {"anies": [{"name": "referenceToUnitGroupDataSet", "value": {"shortDescription": [{"value": "kg", "lang": "en"}], "type": "unit group data set", "refObjectId": "ad38d542-3fe9-439d-9b95-2f5f7752acaf", "uri": "../unitgroups/ad38d542-3fe9-439d-9b95-2f5f7752acaf.xml"}}, {"value": "0.0013", "module": "A1-A3"}, {"value": "4.35E-06", "module": "A4"}, {"value": "4.17E-05", "module": "A5"}, {"value": "0", "module": "B1"}, {"value": "0.000156", "module": "B2"}, {"value": "0", "module": "C1"}, {"value": "2.48E-07", "module": "C2"}, {"module": "C3"}, {"module": "C3", "scenario": "S1"}, {"value": "8.55E-05", "module": "C3", "scenario": "S2"}, {"value": "0.000137", "module": "C3", "scenario": "S3"}, {"module": "C4"}, {"value": "4.13E-05", "module": "C4", "scenario": "S1"}, {"module": "C4", "scenario": "S2"}, {"module": "C4", "scenario": "S3"}, {"value": "-3.37E-05", "module": "D"}, {"value": "0", "module": "D", "scenario": "S1"}, {"value": "-0.00112", "module": "D", "scenario": "S2"}, {"value": "-6.86E-05", "module": "D", "scenario": "S3"}]}, "resolvedFlowVersion": "38.00.000", "flowProperties": [], "typeOfFlow": "Other flow", "classification": {"classHierarchy": "Quantities / Environmental quantities / EPD EN 15804 / LCI indicators", "name": "GaBiCategories"}}, {"dataSetInternalID": 14, "referenceToFlowDataSet": {"shortDescription": [{"value": "Components for re-use (CRU)", "lang": "en"}, {"value": "Komponenten für die Wiederverwendung (CRU)", "lang": "de"}], "type": "flow data set", "refObjectId": "a2b32f97-3fc7-4af2-b209-525bc6426f33", "uri": "../flows/a2b32f97-3fc7-4af2-b209-525bc6426f33.xml"}, "exchange direction": "OUTPUT", "other": {"anies": [{"name": "referenceToUnitGroupDataSet", "value": {"shortDescription": [{"value": "kg", "lang": "en"}], "type": "unit group data set", "refObjectId": "ad38d542-3fe9-439d-9b95-2f5f7752acaf", "uri": "../unitgroups/ad38d542-3fe9-439d-9b95-2f5f7752acaf.xml"}}, {"value": "0", "module": "A1-A3"}, {"value": "0", "module": "A4"}, {"value": "0", "module": "A5"}, {"value": "0", "module": "B1"}, {"value": "0", "module": "B2"}, {"value": "0", "module": "C1"}, {"value": "0", "module": "C2"}, {"module": "C3"}, {"module": "C3", "scenario": "S1"}, {"value": "0", "module": "C3", "scenario": "S2"}, {"value": "0", "module": "C3", "scenario": "S3"}, {"module": "C4"}, {"value": "0", "module": "C4", "scenario": "S1"}, {"module": "C4", "scenario": "S2"}, {"module": "C4", "scenario": "S3"}, {"value": "0", "module": "D"}, {"value": "0", "module": "D", "scenario": "S1"}, {"value": "0", "module": "D", "scenario": "S2"}, {"value": "0", "module": "D", "scenario": "S3"}]}, "resolvedFlowVersion": "38.00.000", "flowProperties": [], "typeOfFlow": "Other flow", "classification": {"classHierarchy": "Quantities / Environmental quantities / EPD EN 15804 / LCI indicators", "name": "GaBiCategories"}}, {"dataSetInternalID": 15, "referenceToFlowDataSet": {"shortDescription": [{"value": "Materials for recycling (MFR)", "lang": "en"}, {"value": "Stoffe zum Recycling (MFR)", "lang": "de"}], "type": "flow data set", "refObjectId": "d7fe48a5-4103-49c8-9aae-b0b5dfdbd6ae", "uri": "../flows/d7fe48a5-4103-49c8-9aae-b0b5dfdbd6ae.xml"}, "exchange direction": "OUTPUT", "other": {"anies": [{"name": "referenceToUnitGroupDataSet", "value": {"shortDescription": [{"value": "kg", "lang": "en"}], "type": "unit group data set", "refObjectId": "ad38d542-3fe9-439d-9b95-2f5f7752acaf", "uri": "../unitgroups/ad38d542-3fe9-439d-9b95-2f5f7752acaf.xml"}}, {"value": "0", "module": "A1-A3"}, {"value": "0", "module": "A4"}, {"value": "0", "module": "A5"}, {"value": "0", "module": "B1"}, {"value": "0", "module": "B2"}, {"value": "0", "module": "C1"}, {"value": "0", "module": "C2"}, {"module": "C3"}, {"module": "C3", "scenario": "S1"}, {"value": "0", "module": "C3", "scenario": "S2"}, {"value": "1.29", "module": "C3", "scenario": "S3"}, {"module": "C4"}, {"value": "0", "module": "C4", "scenario": "S1"}, {"module": "C4", "scenario": "S2"}, {"module": "C4", "scenario": "S3"}, {"value": "0", "module": "D"}, {"value": "0", "module": "D", "scenario": "S1"}, {"value": "0", "module": "D", "scenario": "S2"}, {"value": "0", "module": "D", "scenario": "S3"}]}, "resolvedFlowVersion": "38.00.000", "flowProperties": [], "typeOfFlow": "Other flow", "classification": {"classHierarchy": "Quantities / Environmental quantities / EPD EN 15804 / LCI indicators", "name": "GaBiCategories"}}, {"dataSetInternalID": 16, "referenceToFlowDataSet": {"shortDescription": [{"value": "Materials for energy recovery (MER)", "lang": "en"}, {"value": "Stoffe für die Energierückgewinnung (MER)", "lang": "de"}], "type": "flow data set", "refObjectId": "59a9181c-3aaf-46ee-8b13-2b3723b6e447", "uri": "../flows/59a9181c-3aaf-46ee-8b13-2b3723b6e447.xml"}, "exchange direction": "OUTPUT", "other": {"anies": [{"name": "referenceToUnitGroupDataSet", "value": {"shortDescription": [{"value": "kg", "lang": "en"}], "type": "unit group data set", "refObjectId": "ad38d542-3fe9-439d-9b95-2f5f7752acaf", "uri": "../unitgroups/ad38d542-3fe9-439d-9b95-2f5f7752acaf.xml"}}, {"value": "0", "module": "A1-A3"}, {"value": "0", "module": "A4"}, {"value": "0", "module": "A5"}, {"value": "0", "module": "B1"}, {"value": "0", "module": "B2"}, {"value": "0", "module": "C1"}, {"value": "0", "module": "C2"}, {"module": "C3"}, {"module": "C3", "scenario": "S1"}, {"value": "0", "module": "C3", "scenario": "S2"}, {"value": "0", "module": "C3", "scenario": "S3"}, {"module": "C4"}, {"value": "0", "module": "C4", "scenario": "S1"}, {"module": "C4", "scenario": "S2"}, {"module": "C4", "scenario": "S3"}, {"value": "0", "module": "D"}, {"value": "0", "module": "D", "scenario": "S1"}, {"value": "0", "module": "D", "scenario": "S2"}, {"value": "0", "module": "D", "scenario": "S3"}]}, "resolvedFlowVersion": "38.00.000", "flowProperties": [], "typeOfFlow": "Other flow", "classification": {"classHierarchy": "Quantities / Environmental quantities / EPD EN 15804 / LCI indicators", "name": "GaBiCategories"}}, {"dataSetInternalID": 17, "referenceToFlowDataSet": {"shortDescription": [{"value": "Exported electrical energy (EEE)", "lang": "en"}, {"value": "Exportierte elektrische Energie (EEE)", "lang": "de"}], "type": "flow data set", "refObjectId": "4da0c987-2b76-40d6-9e9e-82a017aaaf29", "uri": "../flows/4da0c987-2b76-40d6-9e9e-82a017aaaf29.xml"}, "exchange direction": "OUTPUT", "other": {"anies": [{"name": "referenceToUnitGroupDataSet", "value": {"shortDescription": [{"value": "MJ", "lang": "en"}], "type": "unit group data set", "refObjectId": "93a60a57-a3c8-11da-a746-0800200c9a66", "uri": "../unitgroups/93a60a57-a3c8-11da-a746-0800200c9a66.xml"}}, {"value": "0", "module": "A1-A3"}, {"value": "0", "module": "A4"}, {"value": "0.112", "module": "A5"}, {"value": "0", "module": "B1"}, {"value": "0", "module": "B2"}, {"value": "0", "module": "C1"}, {"value": "0", "module": "C2"}, {"module": "C3"}, {"module": "C3", "scenario": "S1"}, {"value": "3.73", "module": "C3", "scenario": "S2"}, {"value": "0", "module": "C3", "scenario": "S3"}, {"module": "C4"}, {"value": "0", "module": "C4", "scenario": "S1"}, {"module": "C4", "scenario": "S2"}, {"module": "C4", "scenario": "S3"}, {"value": "0", "module": "D"}, {"value": "0", "module": "D", "scenario": "S1"}, {"value": "0", "module": "D", "scenario": "S2"}, {"value": "0", "module": "D", "scenario": "S3"}]}, "resolvedFlowVersion": "38.00.000", "flowProperties": [], "typeOfFlow": "Other flow", "classification": {"classHierarchy": "Quantities / Environmental quantities / EPD EN 15804 / LCI indicators", "name": "GaBiCategories"}}, {"dataSetInternalID": 18, "referenceToFlowDataSet": {"shortDescription": [{"value": "Exported thermal energy (EET)", "lang": "en"}, {"value": "Exportierte thermische Energie (EET)", "lang": "de"}], "type": "flow data set", "refObjectId": "98daf38a-7a79-46d3-9a37-2b7bd0955810", "uri": "../flows/98daf38a-7a79-46d3-9a37-2b7bd0955810.xml"}, "exchange direction": "OUTPUT", "other": {"anies": [{"name": "referenceToUnitGroupDataSet", "value": {"shortDescription": [{"value": "MJ", "lang": "en"}], "type": "unit group data set", "refObjectId": "93a60a57-a3c8-11da-a746-0800200c9a66", "uri": "../unitgroups/93a60a57-a3c8-11da-a746-0800200c9a66.xml"}}, {"value": "0", "module": "A1-A3"}, {"value": "0", "module": "A4"}, {"value": "0.213", "module": "A5"}, {"value": "0", "module": "B1"}, {"value": "0", "module": "B2"}, {"value": "0", "module": "C1"}, {"value": "0", "module": "C2"}, {"module": "C3"}, {"module": "C3", "scenario": "S1"}, {"value": "7.1", "module": "C3", "scenario": "S2"}, {"value": "37.3", "module": "C3", "scenario": "S3"}, {"module": "C4"}, {"value": "0", "module": "C4", "scenario": "S1"}, {"module": "C4", "scenario": "S2"}, {"module": "C4", "scenario": "S3"}, {"value": "0", "module": "D"}, {"value": "0", "module": "D", "scenario": "S1"}, {"value": "0", "module": "D", "scenario": "S2"}, {"value": "0", "module": "D", "scenario": "S3"}]}, "resolvedFlowVersion": "38.00.000", "flowProperties": [], "typeOfFlow": "Other flow", "classification": {"classHierarchy": "Quantities / Environmental quantities / EPD EN 15804 / LCI indicators", "name": "GaBiCategories"}}]}, "LCIAResults": {"LCIAResult": [{"referenceToLCIAMethodDataSet": {"shortDescription": [{"value": "Global Warming Potential total (GWP-total)", "lang": "en"}, {"value": "Globales Erwärmungspotenzial total (GWP-total)", "lang": "de"}], "type": "LCIA method data set", "refObjectId": "a7ea142a-9749-11ed-a8fc-0242ac120002", "uri": "../lciamethods/a7ea142a-9749-11ed-a8fc-0242ac120002.xml"}, "other": {"anies": [{"name": "referenceToUnitGroupDataSet", "value": {"shortDescription": [{"value": "kg CO_(2) eq", "lang": "en"}], "type": "unit group data set", "refObjectId": "1ebf3012-d0db-4de2-aefd-ef30cedb0be1", "uri": "../unitgroups/1ebf3012-d0db-4de2-aefd-ef30cedb0be1.xml"}}, {"value": "2.76", "module": "A1-A3"}, {"value": "0.2558", "module": "A4"}, {"value": "0.25012", "module": "A5"}, {"value": "0", "module": "B1"}, {"value": "1.508", "module": "B2"}, {"value": "0", "module": "C1"}, {"value": "0.01394", "module": "C2"}, {"module": "C3"}, {"module": "C3", "scenario": "S1"}, {"value": "3.602", "module": "C3", "scenario": "S2"}, {"value": "3.653", "module": "C3", "scenario": "S3"}, {"module": "C4"}, {"value": "1.786", "module": "C4", "scenario": "S1"}, {"module": "C4", "scenario": "S2"}, {"module": "C4", "scenario": "S3"}, {"value": "-0.02444", "module": "D"}, {"value": "0", "module": "D", "scenario": "S1"}, {"value": "-0.8148", "module": "D", "scenario": "S2"}, {"value": "-0.2427", "module": "D", "scenario": "S3"}]}}, {"referenceToLCIAMethodDataSet": {"shortDescription": [{"value": "Global Warming Potential fossil fuels (GWP-fossil)", "lang": "en"}, {"value": "Globales Erwärmungspotenzial fossil (GWP-fossil)", "lang": "de"}], "type": "LCIA method data set", "refObjectId": "a7ea19c0-9749-11ed-a8fc-0242ac120002", "uri": "../lciamethods/a7ea19c0-9749-11ed-a8fc-0242ac120002.xml"}, "other": {"anies": [{"name": "referenceToUnitGroupDataSet", "value": {"shortDescription": [{"value": "kg CO_(2) eq", "lang": "en"}], "type": "unit group data set", "refObjectId": "1ebf3012-d0db-4de2-aefd-ef30cedb0be1", "uri": "../unitgroups/1ebf3012-d0db-4de2-aefd-ef30cedb0be1.xml"}}, {"value": "4.326", "module": "A1-A3"}, {"value": "0.2534", "module": "A4"}, {"value": "0.19724", "module": "A5"}, {"value": "0", "module": "B1"}, {"value": "0.782", "module": "B2"}, {"value": "0", "module": "C1"}, {"value": "0.01378", "module": "C2"}, {"module": "C3"}, {"module": "C3", "scenario": "S1"}, {"value": "1.98", "module": "C3", "scenario": "S2"}, {"value": "2.034", "module": "C3", "scenario": "S3"}, {"module": "C4"}, {"value": "0.2305", "module": "C4", "scenario": "S1"}, {"module": "C4", "scenario": "S2"}, {"module": "C4", "scenario": "S3"}, {"value": "-0.02433", "module": "D"}, {"value": "0", "module": "D", "scenario": "S1"}, {"value": "-0.8111", "module": "D", "scenario": "S2"}, {"value": "-0.2427", "module": "D", "scenario": "S3"}]}}, {"referenceToLCIAMethodDataSet": {"shortDescription": [{"value": "Global Warming Potential biogenic (GWP-biogenic)", "lang": "en"}, {"value": "Globales Erwärmungspotenzial biogen (GWP-biogenic)", "lang": "de"}], "type": "LCIA method data set", "refObjectId": "a7ea186c-9749-11ed-a8fc-0242ac120002", "uri": "../lciamethods/a7ea186c-9749-11ed-a8fc-0242ac120002.xml"}, "other": {"anies": [{"name": "referenceToUnitGroupDataSet", "value": {"shortDescription": [{"value": "kg CO_(2) eq", "lang": "en"}], "type": "unit group data set", "refObjectId": "1ebf3012-d0db-4de2-aefd-ef30cedb0be1", "uri": "../unitgroups/1ebf3012-d0db-4de2-aefd-ef30cedb0be1.xml"}}, {"value": "-1.704", "module": "A1-A3"}, {"value": "0.0005106", "module": "A4"}, {"value": "0.04869", "module": "A5"}, {"value": "0", "module": "B1"}, {"value": "0.01748", "module": "B2"}, {"value": "0", "module": "C1"}, {"value": "3.225E-05", "module": "C2"}, {"module": "C3"}, {"module": "C3", "scenario": "S1"}, {"value": "1.623", "module": "C3", "scenario": "S2"}, {"value": "1.618", "module": "C3", "scenario": "S3"}, {"module": "C4"}, {"value": "1.555", "module": "C4", "scenario": "S1"}, {"module": "C4", "scenario": "S2"}, {"module": "C4", "scenario": "S3"}, {"value": "-0.0001091", "module": "D"}, {"value": "0", "module": "D", "scenario": "S1"}, {"value": "-0.003637", "module": "D", "scenario": "S2"}, {"value": "0.0001814", "module": "D", "scenario": "S3"}]}}, {"referenceToLCIAMethodDataSet": {"shortDescription": [{"value": "Global Warming Potential luluc (GWP-luluc)", "lang": "en"}, {"value": "Globales Erwärmungspotenzial luluc (GWP-luluc)", "lang": "de"}], "type": "LCIA method data set", "refObjectId": "a7ea1ae2-9749-11ed-a8fc-0242ac120002", "uri": "../lciamethods/a7ea1ae2-9749-11ed-a8fc-0242ac120002.xml"}, "other": {"anies": [{"name": "referenceToUnitGroupDataSet", "value": {"shortDescription": [{"value": "kg CO_(2) eq", "lang": "en"}], "type": "unit group data set", "refObjectId": "1ebf3012-d0db-4de2-aefd-ef30cedb0be1", "uri": "../unitgroups/1ebf3012-d0db-4de2-aefd-ef30cedb0be1.xml"}}, {"value": "0.1374", "module": "A1-A3"}, {"value": "0.001844", "module": "A4"}, {"value": "0.0041883", "module": "A5"}, {"value": "0", "module": "B1"}, {"value": "0.7086", "module": "B2"}, {"value": "0", "module": "C1"}, {"value": "0.0001305", "module": "C2"}, {"module": "C3"}, {"module": "C3", "scenario": "S1"}, {"value": "0.0002138", "module": "C3", "scenario": "S2"}, {"value": "0.0005416", "module": "C3", "scenario": "S3"}, {"module": "C4"}, {"value": "0.0001925", "module": "C4", "scenario": "S1"}, {"module": "C4", "scenario": "S2"}, {"module": "C4", "scenario": "S3"}, {"value": "-1.564E-06", "module": "D"}, {"value": "0", "module": "D", "scenario": "S1"}, {"value": "-5.214E-05", "module": "D", "scenario": "S2"}, {"value": "-0.0001627", "module": "D", "scenario": "S3"}]}}, {"referenceToLCIAMethodDataSet": {"shortDescription": [{"value": "Depletion potential of the stratospheric ozone layer (ODP)", "lang": "en"}, {"value": "Abbau Potential der stratosphärischen Ozonschicht (ODP)", "lang": "de"}], "type": "LCIA method data set", "refObjectId": "b5c629d6-def3-11e6-bf01-fe55135034f3", "uri": "../lciamethods/b5c629d6-def3-11e6-bf01-fe55135034f3.xml"}, "other": {"anies": [{"name": "referenceToUnitGroupDataSet", "value": {"shortDescription": [{"value": "kg CFC11 eq", "lang": "en"}], "type": "unit group data set", "refObjectId": "d9e957c9-7309-4474-bf3a-7777df6c4e5b", "uri": "../unitgroups/d9e957c9-7309-4474-bf3a-7777df6c4e5b.xml"}}, {"value": "7.149E-08", "module": "A1-A3"}, {"value": "2.144E-14", "module": "A4"}, {"value": "2.144707102E-09", "module": "A5"}, {"value": "0", "module": "B1"}, {"value": "1.233E-07", "module": "B2"}, {"value": "0", "module": "C1"}, {"value": "1.233E-15", "module": "C2"}, {"module": "C3"}, {"module": "C3", "scenario": "S1"}, {"value": "2.139E-13", "module": "C3", "scenario": "S2"}, {"value": "4.981E-13", "module": "C3", "scenario": "S3"}, {"module": "C4"}, {"value": "3.929E-13", "module": "C4", "scenario": "S1"}, {"module": "C4", "scenario": "S2"}, {"module": "C4", "scenario": "S3"}, {"value": "-1.858E-13", "module": "D"}, {"value": "0", "module": "D", "scenario": "S1"}, {"value": "-6.193E-12", "module": "D", "scenario": "S2"}, {"value": "-5.907E-13", "module": "D", "scenario": "S3"}]}}, {"referenceToLCIAMethodDataSet": {"shortDescription": [{"value": "Acidification potential of land and water (AP)", "lang": "en"}, {"value": "Versauerungspotenzial von Boden und Wasser (AP)", "lang": "de"}], "type": "LCIA method data set", "refObjectId": "b5c611c6-def3-11e6-bf01-fe55135034f3", "uri": "../lciamethods/b5c611c6-def3-11e6-bf01-fe55135034f3.xml"}, "other": {"anies": [{"name": "referenceToUnitGroupDataSet", "value": {"shortDescription": [{"value": "mol H^(+) eq", "lang": "en"}], "type": "unit group data set", "refObjectId": "42e089ac-92bf-4bf2-8ca1-5fc40d18f2ed", "uri": "../unitgroups/42e089ac-92bf-4bf2-8ca1-5fc40d18f2ed.xml"}}, {"value": "0.03867", "module": "A1-A3"}, {"value": "0.003204", "module": "A4"}, {"value": "0.0013147", "module": "A5"}, {"value": "0", "module": "B1"}, {"value": "0.002109", "module": "B2"}, {"value": "0", "module": "C1"}, {"value": "8.667E-05", "module": "C2"}, {"module": "C3"}, {"module": "C3", "scenario": "S1"}, {"value": "0.001865", "module": "C3", "scenario": "S2"}, {"value": "0.002114", "module": "C3", "scenario": "S3"}, {"module": "C4"}, {"value": "0.0007014", "module": "C4", "scenario": "S1"}, {"module": "C4", "scenario": "S2"}, {"module": "C4", "scenario": "S3"}, {"value": "-2.999E-05", "module": "D"}, {"value": "0", "module": "D", "scenario": "S1"}, {"value": "-0.0009995", "module": "D", "scenario": "S2"}, {"value": "-0.0008151", "module": "D", "scenario": "S3"}]}}, {"referenceToLCIAMethodDataSet": {"shortDescription": [{"value": "Eutrophication potential aquatic freshwater (EP-freshwater)", "lang": "en"}, {"value": "Eutrophierungspotenzial Süßwasser (EP-freshwater)", "lang": "de"}], "type": "LCIA method data set", "refObjectId": "b53ec18f-7377-4ad3-86eb-cc3f4f276b2b", "uri": "../lciamethods/b53ec18f-7377-4ad3-86eb-cc3f4f276b2b.xml"}, "other": {"anies": [{"name": "referenceToUnitGroupDataSet", "value": {"shortDescription": [{"value": "kg P eq", "lang": "en"}], "type": "unit group data set", "refObjectId": "0429039d-a61d-4590-ba67-aa4a20a810a1", "uri": "../unitgroups/0429039d-a61d-4590-ba67-aa4a20a810a1.xml"}}, {"value": "0.001208", "module": "A1-A3"}, {"value": "7.389E-07", "module": "A4"}, {"value": "3.628519E-05", "module": "A5"}, {"value": "0", "module": "B1"}, {"value": "2.676E-05", "module": "B2"}, {"value": "0", "module": "C1"}, {"value": "5.136E-08", "module": "C2"}, {"module": "C3"}, {"module": "C3", "scenario": "S1"}, {"value": "7.076E-07", "module": "C3", "scenario": "S2"}, {"value": "8.929E-07", "module": "C3", "scenario": "S3"}, {"module": "C4"}, {"value": "4.501E-05", "module": "C4", "scenario": "S1"}, {"module": "C4", "scenario": "S2"}, {"module": "C4", "scenario": "S3"}, {"value": "-3.837E-08", "module": "D"}, {"value": "0", "module": "D", "scenario": "S1"}, {"value": "-1.279E-06", "module": "D", "scenario": "S2"}, {"value": "-3.612E-07", "module": "D", "scenario": "S3"}]}}, {"referenceToLCIAMethodDataSet": {"shortDescription": [{"value": "Eutrophication potential aquatic marine (EP-marine)", "lang": "en"}, {"value": "Eutrophierungspotenzial Salzwasser (EP-marine)", "lang": "de"}], "type": "LCIA method data set", "refObjectId": "b5c619fa-def3-11e6-bf01-fe55135034f3", "uri": "../lciamethods/b5c619fa-def3-11e6-bf01-fe55135034f3.xml"}, "other": {"anies": [{"name": "referenceToUnitGroupDataSet", "value": {"shortDescription": [{"value": "kg N eq", "lang": "en"}], "type": "unit group data set", "refObjectId": "d05bb823-ecdf-4686-8c40-bf1d9257859f", "uri": "../unitgroups/d05bb823-ecdf-4686-8c40-bf1d9257859f.xml"}}, {"value": "0.01512", "module": "A1-A3"}, {"value": "0.001085", "module": "A4"}, {"value": "0.00051346", "module": "A5"}, {"value": "0", "module": "B1"}, {"value": "0.0005463", "module": "B2"}, {"value": "0", "module": "C1"}, {"value": "4.247E-05", "module": "C2"}, {"module": "C3"}, {"module": "C3", "scenario": "S1"}, {"value": "0.0008653", "module": "C3", "scenario": "S2"}, {"value": "0.0009793", "module": "C3", "scenario": "S3"}, {"module": "C4"}, {"value": "0.0001607", "module": "C4", "scenario": "S1"}, {"module": "C4", "scenario": "S2"}, {"module": "C4", "scenario": "S3"}, {"value": "-8.828E-06", "module": "D"}, {"value": "0", "module": "D", "scenario": "S1"}, {"value": "-0.0002943", "module": "D", "scenario": "S2"}, {"value": "-0.000276", "module": "D", "scenario": "S3"}]}}, {"referenceToLCIAMethodDataSet": {"shortDescription": [{"value": "Eutrophication potential terrestrial (EP-terrestrial)", "lang": "en"}, {"value": "Eutrophierungspotenzial Land (EP-terrestrial)", "lang": "de"}], "type": "LCIA method data set", "refObjectId": "b5c614d2-def3-11e6-bf01-fe55135034f3", "uri": "../lciamethods/b5c614d2-def3-11e6-bf01-fe55135034f3.xml"}, "other": {"anies": [{"name": "referenceToUnitGroupDataSet", "value": {"shortDescription": [{"value": "mol N eq", "lang": "en"}], "type": "unit group data set", "refObjectId": "71b4d617-0ec9-4d3f-b65e-e438940c2401", "uri": "../unitgroups/71b4d617-0ec9-4d3f-b65e-e438940c2401.xml"}}, {"value": "0.1531", "module": "A1-A3"}, {"value": "0.01197", "module": "A4"}, {"value": "0.0052628", "module": "A5"}, {"value": "0", "module": "B1"}, {"value": "0.008128", "module": "B2"}, {"value": "0", "module": "C1"}, {"value": "0.0004712", "module": "C2"}, {"module": "C3"}, {"module": "C3", "scenario": "S1"}, {"value": "0.009858", "module": "C3", "scenario": "S2"}, {"value": "0.01112", "module": "C3", "scenario": "S3"}, {"module": "C4"}, {"value": "0.001764", "module": "C4", "scenario": "S1"}, {"module": "C4", "scenario": "S2"}, {"module": "C4", "scenario": "S3"}, {"value": "-9.459E-05", "module": "D"}, {"value": "0", "module": "D", "scenario": "S1"}, {"value": "-0.003153", "module": "D", "scenario": "S2"}, {"value": "-0.003026", "module": "D", "scenario": "S3"}]}}, {"referenceToLCIAMethodDataSet": {"shortDescription": [{"value": "Formation potential of tropospheric ozone photochemical oxidants (POCP)", "lang": "en"}, {"value": "Bildungspotential für troposphärisches Ozon (POCP)", "lang": "de"}], "type": "LCIA method data set", "refObjectId": "b5c610fe-def3-11e6-bf01-fe55135034f3", "uri": "../lciamethods/b5c610fe-def3-11e6-bf01-fe55135034f3.xml"}, "other": {"anies": [{"name": "referenceToUnitGroupDataSet", "value": {"shortDescription": [{"value": "kg NMVOC eq", "lang": "en"}], "type": "unit group data set", "refObjectId": "d27c25f8-fbc1-44c6-b47b-4adbae4199c6", "uri": "../unitgroups/d27c25f8-fbc1-44c6-b47b-4adbae4199c6.xml"}}, {"value": "0.01327", "module": "A1-A3"}, {"value": "0.002511", "module": "A4"}, {"value": "0.0005431", "module": "A5"}, {"value": "1.19E-05", "module": "B1"}, {"value": "0.003011", "module": "B2"}, {"value": "0", "module": "C1"}, {"value": "8.033E-05", "module": "C2"}, {"module": "C3"}, {"module": "C3", "scenario": "S1"}, {"value": "0.00224", "module": "C3", "scenario": "S2"}, {"value": "0.002462", "module": "C3", "scenario": "S3"}, {"module": "C4"}, {"value": "0.0005104", "module": "C4", "scenario": "S1"}, {"module": "C4", "scenario": "S2"}, {"module": "C4", "scenario": "S3"}, {"value": "-2.463E-05", "module": "D"}, {"value": "0", "module": "D", "scenario": "S1"}, {"value": "-0.0008209", "module": "D", "scenario": "S2"}, {"value": "-0.0008402", "module": "D", "scenario": "S3"}]}}, {"referenceToLCIAMethodDataSet": {"shortDescription": [{"value": "Abiotic depletion potential for non fossil resources (ADPE)", "lang": "en"}, {"value": "Potenzial für den abiotischen Abbau nicht fossiler Ressourcen (ADPE)", "lang": "de"}], "type": "LCIA method data set", "refObjectId": "b2ad6494-c78d-11e6-9d9d-cec0c932ce01", "uri": "../lciamethods/b2ad6494-c78d-11e6-9d9d-cec0c932ce01.xml"}, "other": {"anies": [{"name": "referenceToUnitGroupDataSet", "value": {"shortDescription": [{"value": "kg Sb eq", "lang": "en"}], "type": "unit group data set", "refObjectId": "54ccd2d9-a32a-4fc2-923d-f2c8c93e89d4", "uri": "../unitgroups/54ccd2d9-a32a-4fc2-923d-f2c8c93e89d4.xml"}}, {"value": "4.745E-06", "module": "A1-A3"}, {"value": "1.346E-08", "module": "A4"}, {"value": "1.4325E-07", "module": "A5"}, {"value": "0", "module": "B1"}, {"value": "7.173E-07", "module": "B2"}, {"value": "0", "module": "C1"}, {"value": "9.148E-10", "module": "C2"}, {"module": "C3"}, {"module": "C3", "scenario": "S1"}, {"value": "1.548E-08", "module": "C3", "scenario": "S2"}, {"value": "2.012E-08", "module": "C3", "scenario": "S3"}, {"module": "C4"}, {"value": "6.183E-09", "module": "C4", "scenario": "S1"}, {"module": "C4", "scenario": "S2"}, {"module": "C4", "scenario": "S3"}, {"value": "-1.705E-09", "module": "D"}, {"value": "0", "module": "D", "scenario": "S1"}, {"value": "-5.684E-08", "module": "D", "scenario": "S2"}, {"value": "-1.032E-08", "module": "D", "scenario": "S3"}]}}, {"referenceToLCIAMethodDataSet": {"shortDescription": [{"value": "Abiotic depletion potential for fossil resources (ADPF)", "lang": "en"}, {"value": "Potenzial für den abiotischen Abbau fossiler Brennstoffe (ADPF)", "lang": "de"}], "type": "LCIA method data set", "refObjectId": "b2ad6110-c78d-11e6-9d9d-cec0c932ce01", "uri": "../lciamethods/b2ad6110-c78d-11e6-9d9d-cec0c932ce01.xml"}, "other": {"anies": [{"name": "referenceToUnitGroupDataSet", "value": {"shortDescription": [{"value": "MJ", "lang": "en"}], "type": "unit group data set", "refObjectId": "93a60a57-a3c8-11da-a746-0800200c9a66", "uri": "../unitgroups/93a60a57-a3c8-11da-a746-0800200c9a66.xml"}}, {"value": "77.55", "module": "A1-A3"}, {"value": "3.424", "module": "A4"}, {"value": "2.4988", "module": "A5"}, {"value": "0", "module": "B1"}, {"value": "13.83", "module": "B2"}, {"value": "0", "module": "C1"}, {"value": "0.1915", "module": "C2"}, {"module": "C3"}, {"module": "C3", "scenario": "S1"}, {"value": "2.1", "module": "C3", "scenario": "S2"}, {"value": "2.9", "module": "C3", "scenario": "S3"}, {"module": "C4"}, {"value": "3.49", "module": "C4", "scenario": "S1"}, {"module": "C4", "scenario": "S2"}, {"module": "C4", "scenario": "S3"}, {"value": "-0.4481", "module": "D"}, {"value": "0", "module": "D", "scenario": "S1"}, {"value": "-14.94", "module": "D", "scenario": "S2"}, {"value": "-40.36", "module": "D", "scenario": "S3"}]}}, {"referenceToLCIAMethodDataSet": {"shortDescription": [{"value": "Water use (WDP)", "lang": "en"}, {"value": "Wassernutzung (WDP)", "lang": "de"}], "type": "LCIA method data set", "refObjectId": "b2ad66ce-c78d-11e6-9d9d-cec0c932ce01", "uri": "../lciamethods/b2ad66ce-c78d-11e6-9d9d-cec0c932ce01.xml"}, "other": {"anies": [{"name": "referenceToUnitGroupDataSet", "value": {"shortDescription": [{"value": "m^(3) world eq deprived", "lang": "en"}], "type": "unit group data set", "refObjectId": "6ae2df01-888e-46c8-b17d-49fa3869b476", "uri": "../unitgroups/6ae2df01-888e-46c8-b17d-49fa3869b476.xml"}}, {"value": "69.03", "module": "A1-A3"}, {"value": "0.002391", "module": "A4"}, {"value": "2.08638", "module": "A5"}, {"value": "0", "module": "B1"}, {"value": "0.3383", "module": "B2"}, {"value": "0", "module": "C1"}, {"value": "0.0001623", "module": "C2"}, {"module": "C3"}, {"module": "C3", "scenario": "S1"}, {"value": "0.5135", "module": "C3", "scenario": "S2"}, {"value": "0.5173", "module": "C3", "scenario": "S3"}, {"module": "C4"}, {"value": "-0.003301", "module": "C4", "scenario": "S1"}, {"module": "C4", "scenario": "S2"}, {"module": "C4", "scenario": "S3"}, {"value": "-0.002251", "module": "D"}, {"value": "0", "module": "D", "scenario": "S1"}, {"value": "-0.07504", "module": "D", "scenario": "S2"}, {"value": "-0.02934", "module": "D", "scenario": "S3"}]}}, {"referenceToLCIAMethodDataSet": {"shortDescription": [{"value": "Incidence of disease due to PM emissions (PM)", "lang": "en"}, {"value": "Auftreten von Krankheiten aufgrund von Feinstaubemissionen (PM)", "lang": "de"}], "type": "LCIA method data set", "refObjectId": "b5c602c6-def3-11e6-bf01-fe55135034f3", "uri": "../lciamethods/b5c602c6-def3-11e6-bf01-fe55135034f3.xml"}, "other": {"anies": [{"name": "referenceToUnitGroupDataSet", "value": {"shortDescription": [{"value": "Disease incidence", "lang": "en"}], "type": "unit group data set", "refObjectId": "3883559b-648f-4afc-8ba2-0bd24f3affa3", "uri": "../unitgroups/3883559b-648f-4afc-8ba2-0bd24f3affa3.xml"}}, {"value": "3.51E-07", "module": "A1-A3"}, {"value": "4.31E-08", "module": "A4"}, {"value": "1.224E-08", "module": "A5"}, {"value": "0", "module": "B1"}, {"value": "2.4E-07", "module": "B2"}, {"value": "0", "module": "C1"}, {"value": "5.45E-10", "module": "C2"}, {"module": "C3"}, {"module": "C3", "scenario": "S1"}, {"value": "1.37E-08", "module": "C3", "scenario": "S2"}, {"value": "1.53E-08", "module": "C3", "scenario": "S3"}, {"module": "C4"}, {"value": "6.8E-09", "module": "C4", "scenario": "S1"}, {"module": "C4", "scenario": "S2"}, {"module": "C4", "scenario": "S3"}, {"value": "-2.55E-10", "module": "D"}, {"value": "0", "module": "D", "scenario": "S1"}, {"value": "-8.48E-09", "module": "D", "scenario": "S2"}, {"value": "-2.59E-08", "module": "D", "scenario": "S3"}]}}, {"referenceToLCIAMethodDataSet": {"shortDescription": [{"value": "Human exposure efficiency relative to U235 (IR)", "lang": "en"}, {"value": "Wirkung durch Exposition des Menschen mit U235 (IR)", "lang": "de"}], "type": "LCIA method data set", "refObjectId": "b5c632be-def3-11e6-bf01-fe55135034f3", "uri": "../lciamethods/b5c632be-def3-11e6-bf01-fe55135034f3.xml"}, "other": {"anies": [{"name": "referenceToUnitGroupDataSet", "value": {"shortDescription": [{"value": "kBq U235 eq", "lang": "en"}], "type": "unit group data set", "refObjectId": "456b05bf-1415-44a9-9993-02452f554c09", "uri": "../unitgroups/456b05bf-1415-44a9-9993-02452f554c09.xml"}}, {"value": "0.504", "module": "A1-A3"}, {"value": "0.000627", "module": "A4"}, {"value": "0.015531", "module": "A5"}, {"value": "0", "module": "B1"}, {"value": "0.0414", "module": "B2"}, {"value": "0", "module": "C1"}, {"value": "3.58E-05", "module": "C2"}, {"module": "C3"}, {"module": "C3", "scenario": "S1"}, {"value": "0.013", "module": "C3", "scenario": "S2"}, {"value": "0.0216", "module": "C3", "scenario": "S3"}, {"module": "C4"}, {"value": "0.00611", "module": "C4", "scenario": "S1"}, {"module": "C4", "scenario": "S2"}, {"module": "C4", "scenario": "S3"}, {"value": "-0.0056", "module": "D"}, {"value": "0", "module": "D", "scenario": "S1"}, {"value": "-0.187", "module": "D", "scenario": "S2"}, {"value": "-0.00659", "module": "D", "scenario": "S3"}]}}, {"referenceToLCIAMethodDataSet": {"shortDescription": [{"value": "Comparative toxic unit for ecosystems (ETP-fw)", "lang": "en"}, {"value": "Toxizitätsvergleichseinheit für Ökosysteme (ETP-fw)", "lang": "de"}], "type": "LCIA method data set", "refObjectId": "ee1082d1-b0f7-43ca-a1f0-21e2a4a74511", "uri": "../lciamethods/ee1082d1-b0f7-43ca-a1f0-21e2a4a74511.xml"}, "other": {"anies": [{"name": "referenceToUnitGroupDataSet", "value": {"shortDescription": [{"value": "CTUe", "lang": "en"}], "type": "unit group data set", "refObjectId": "aa959ded-f1eb-4efb-9c5c-2d60be36b3e6", "uri": "../unitgroups/aa959ded-f1eb-4efb-9c5c-2d60be36b3e6.xml"}}, {"value": "33.2", "module": "A1-A3"}, {"value": "2.41", "module": "A4"}, {"value": "1.105", "module": "A5"}, {"value": "0.000102", "module": "B1"}, {"value": "5.72", "module": "B2"}, {"value": "0", "module": "C1"}, {"value": "0.135", "module": "C2"}, {"module": "C3"}, {"module": "C3", "scenario": "S1"}, {"value": "1.08", "module": "C3", "scenario": "S2"}, {"value": "1.51", "module": "C3", "scenario": "S3"}, {"module": "C4"}, {"value": "2.98", "module": "C4", "scenario": "S1"}, {"module": "C4", "scenario": "S2"}, {"module": "C4", "scenario": "S3"}, {"value": "-0.0609", "module": "D"}, {"value": "0", "module": "D", "scenario": "S1"}, {"value": "-2.03", "module": "D", "scenario": "S2"}, {"value": "-15.2", "module": "D", "scenario": "S3"}]}}, {"referenceToLCIAMethodDataSet": {"shortDescription": [{"value": "Comparative toxic unit for humans (carcinogenic) (HTP-c)", "lang": "en"}, {"value": "Toxizitätsvergleichseinheit für Menschen (krebserregend) (HTP-c)", "lang": "de"}], "type": "LCIA method data set", "refObjectId": "2299222a-bbd8-474f-9d4f-4dd1f18aea7c", "uri": "../lciamethods/2299222a-bbd8-474f-9d4f-4dd1f18aea7c.xml"}, "other": {"anies": [{"name": "referenceToUnitGroupDataSet", "value": {"shortDescription": [{"value": "CTUh", "lang": "en"}], "type": "unit group data set", "refObjectId": "d4c9523e-2d7e-49fd-8469-998f547d3a70", "uri": "../unitgroups/d4c9523e-2d7e-49fd-8469-998f547d3a70.xml"}}, {"value": "2.82E-09", "module": "A1-A3"}, {"value": "4.78E-11", "module": "A4"}, {"value": "8.77E-11", "module": "A5"}, {"value": "0", "module": "B1"}, {"value": "2.19E-09", "module": "B2"}, {"value": "0", "module": "C1"}, {"value": "2.73E-12", "module": "C2"}, {"module": "C3"}, {"module": "C3", "scenario": "S1"}, {"value": "5.24E-11", "module": "C3", "scenario": "S2"}, {"value": "6.39E-11", "module": "C3", "scenario": "S3"}, {"module": "C4"}, {"value": "1.53E-10", "module": "C4", "scenario": "S1"}, {"module": "C4", "scenario": "S2"}, {"module": "C4", "scenario": "S3"}, {"value": "-4.92E-12", "module": "D"}, {"value": "0", "module": "D", "scenario": "S1"}, {"value": "-1.64E-10", "module": "D", "scenario": "S2"}, {"value": "-6.78E-11", "module": "D", "scenario": "S3"}]}}, {"referenceToLCIAMethodDataSet": {"shortDescription": [{"value": "Comparative toxic unit for humans (noncarcinogenic) (HTP-nc)", "lang": "en"}, {"value": "Toxizitätsvergleichseinheit für Menschen (nicht krebserregend) (HTP-nc)", "lang": "de"}], "type": "LCIA method data set", "refObjectId": "3af763a5-b7a1-48c9-9cee-1f223481fcef", "uri": "../lciamethods/3af763a5-b7a1-48c9-9cee-1f223481fcef.xml"}, "other": {"anies": [{"name": "referenceToUnitGroupDataSet", "value": {"shortDescription": [{"value": "CTUh", "lang": "en"}], "type": "unit group data set", "refObjectId": "d4c9523e-2d7e-49fd-8469-998f547d3a70", "uri": "../unitgroups/d4c9523e-2d7e-49fd-8469-998f547d3a70.xml"}}, {"value": "1.5E-07", "module": "A1-A3"}, {"value": "1.99E-09", "module": "A4"}, {"value": "4.649E-09", "module": "A5"}, {"value": "7.4E-13", "module": "B1"}, {"value": "2.47E-08", "module": "B2"}, {"value": "0", "module": "C1"}, {"value": "1.2E-10", "module": "C2"}, {"module": "C3"}, {"module": "C3", "scenario": "S1"}, {"value": "2.82E-09", "module": "C3", "scenario": "S2"}, {"value": "3.19E-09", "module": "C3", "scenario": "S3"}, {"module": "C4"}, {"value": "1.22E-08", "module": "C4", "scenario": "S1"}, {"module": "C4", "scenario": "S2"}, {"module": "C4", "scenario": "S3"}, {"value": "-1.22E-10", "module": "D"}, {"value": "0", "module": "D", "scenario": "S1"}, {"value": "-4.08E-09", "module": "D", "scenario": "S2"}, {"value": "-2.55E-09", "module": "D", "scenario": "S3"}]}}, {"referenceToLCIAMethodDataSet": {"shortDescription": [{"value": "Soil quality index (SQP)", "lang": "en"}, {"value": "Bodenqualitätsindex (SQP)", "lang": "de"}], "type": "LCIA method data set", "refObjectId": "b2ad6890-c78d-11e6-9d9d-cec0c932ce01", "uri": "../lciamethods/b2ad6890-c78d-11e6-9d9d-cec0c932ce01.xml"}, "other": {"anies": [{"name": "referenceToUnitGroupDataSet", "value": {"shortDescription": [{"value": "SQP", "lang": "en"}], "type": "unit group data set", "refObjectId": "f130951c-e67f-4f7f-8dd4-665de3974e18", "uri": "../unitgroups/f130951c-e67f-4f7f-8dd4-665de3974e18.xml"}}, {"module": "A1-A3"}, {"module": "A4"}, {"module": "A5"}, {"module": "B1"}, {"module": "B2"}, {"module": "C1"}, {"module": "C2"}, {"module": "C3"}, {"module": "C3", "scenario": "S1"}, {"module": "C3", "scenario": "S2"}, {"module": "C3", "scenario": "S3"}, {"module": "C4"}, {"module": "C4", "scenario": "S1"}, {"module": "C4", "scenario": "S2"}, {"module": "C4", "scenario": "S3"}, {"module": "D"}, {"module": "D", "scenario": "S1"}, {"module": "D", "scenario": "S2"}, {"module": "D", "scenario": "S3"}]}}]}, "otherAttributes": {"{http://www.indata.network/EPD/2019}epd-version": "1.2"}, "version": "1.1", "locations": "../ILCDLocations.xml"}