{"processInformation": {"dataSetInformation": {"UUID": "fbf5dbfe-7338-4c8d-b195-c68074be581a", "name": {"baseName": [{"value": "VELUX wooden roof windows with glazing configuration 62 and 62D", "lang": "en"}, {"value": "VELUX Holzdachfenster mit Verglasungskonfiguration 62 und 62D", "lang": "de"}], "functionalUnitFlowProperties": [{"lang": "en"}]}, "classificationInformation": {"classification": [{"class": [{"value": "Komponenten von Fenstern und Vorhangfassaden", "level": 0, "classId": "7"}, {"value": "Fenster", "level": 1, "classId": "7.8"}, {"value": "Holzfenster", "level": 2, "classId": "7.8.01"}], "name": "OEKOBAU.DAT"}, {"class": [{"value": "02 Building products", "level": 0}, {"value": "Doors, windows, shutters, and related products", "level": 1}, {"value": "Windows and doors ", "level": 2}], "name": "IBUCategories"}]}, "generalComment": [{"value": "The VELUX wooden roof windows are skylight window products for sale in the European market. The product family covers a range of product varieties as specified in the table below. All windows have a wooden frame/sash. Some windows can be opened (venting), while others cannot be opened (fixed). In addition, the windows consist of 4 different hinge-functionalities (pivot-hung, top-hung, side-hung, bottom-hung). The handles and handlebars are made of aluminium, while the hinges are made of steel (galvanised, stainless). Some of the window varieties can be used in conjunction with electric or solar window operators for automatic opening and closing, while other windows are opened and closed manually. The calculations are based on the representative window type named GPL. In the LCA, the GPL was assessed to be a conservative choice for a representative window type.\n\nThe glass panes are with double and triple glazing (2-layer and 3-layer glazing unit) and the glass configurations 62 and 62 D are covered by the EPD. The glass panes have cavities filled with Argon or Krypton gas. The EPD is based on the glazing unit configuration 62 (assessed to be a conservative choice over 62 D).\n\nOnly the window modules are included, which means that any applied window operators, installation products, accessories, etc. are not part of the EPD. These are available as separate EPDs, that can be used in combination with this EPD.\n\n\n1 2-layer glazing options: 62 D, 3-layer glazing options: 62", "lang": "en"}, {"value": "Die VELUX Dachfenster aus Holz sind Oberlichtfensterprodukte, die auf dem europäischen Markt verkauft werden. Die Produktfamilie umfasst eine Reihe von Produktvarianten. Alle Fenster haben einen Holzrahmen/Flügel. Einige Fenster können geöffnet werden (Lüften), während andere nicht geöffnet werden können (festgelegt). Darüber hinaus verfügen die Fenster über 4 verschiedene Scharnierfunktionalitäten (Kipp-, Klapp-, Dreh- und Kippfenster). Die Griffe und Lenkstangen bestehen aus Aluminium, während die Scharniere aus Stahl (verzinkt, rostfrei) bestehen. Einige der Fenstervarianten können in Verbindung mit elektrischen oder solaren Fensterantrieben zum automatischen Öffnen und Schließen verwendet werden, während andere Fenster manuell geöffnet und geschlossen werden. Die Berechnungen basieren auf dem repräsentativen Fenstertyp namens GPL. In der Ökobilanz wurde die GPL als konservative Wahl für einen repräsentativen Fenstertyp bewertet. Die Glasscheiben sind mit Doppel- und Dreifachverglasung (2-fach- und 3-fach-Verglasung) ausgestattet und die Glaskonfigurationen 62 und 62D fallen unter die EPD. Die Glasscheiben haben Hohlräume, die mit Argon- oder Kryptongas gefüllt sind. Die EPD basiert auf der Verglasungseinheitskonfiguration 62 (die als konservative Wahl gegenüber 62D eingeschätzt wird). Berücksichtigt werden ausschließlich die Fenstermodule, d. h. etwaige eingesetzte Fensterantriebe, Montageprodukte, Zubehör etc. sind nicht Bestandteil der EPD. Diese sind als separate EPDs erhältlich, die in Kombination mit dieser EPD verwendet werden können.", "lang": "de"}]}, "quantitativeReference": {"referenceToReferenceFlow": [0]}, "time": {"referenceYear": 2024, "dataSetValidUntil": 2029, "other": {"anies": [{"name": "publicationDateOfEPD", "value": 1710115200000}]}}, "geography": {"locationOfOperationSupplyOrProduction": {"location": "RER"}}, "technology": {"technologyDescriptionAndIncludedProcesses": [{"value": "The main components of the standard wooden roof window are the glazing unit (made of mainly laminated and tempered glass), wooden frames/sashes (made of wood), hinges (made of steel) and handles/handlebars (made of aluminium). The packaging of the products consists of mostly cardboard along paper insert and galvanised steel. The wooden components (sashes, frames) are produced internally in VELUX facilities, located in Hungary, Poland, and France. VELUX receives sawn pine wood (dried) and process it (sawing, cutting etc.) into lamellas of different quality. The lamellas are then glued together (lamination) and processed into profiles (cutting them into the correct size, cladding, drilling etc.). For the glazing units, VELUX receives the glazing units components from suppliers and produces the final glazing units in sites located in Hungary, Denmark, France, and Germany. After their production, the glazing units join the window assembly process. Finally, the frames/sashes, glazing unit and the rest of the components (delivered by suppliers) are transported to VELUX assembly sites in Poland, Denmark, France and Germany, where they are assembled into the final window product. \nTechnical data: \nThe Declaration of Performance including relevant technical specifications and test methods/test standards can be downloaded from the website www.velux.com/ce\n\nThe performance values are specific for each standard wooden roof window variant covered by the EPD. The declared values in the table relate to the reference product including the variant GGL with triple-glazed configuration 62 (GGL --62). For other covered product variants, specific values can be selected at the bottom of the above-mentioned download page. \nDeclared unit: \nMultiple product dimensions are represented by this EPD as specified in the product description. The declared unit is 1 m2 wooden roof window calculated based on the size 1.34 m x 1.40 m (UK08), which is the closest available size to the reference window size (1.23 m x 1.48 m based on EN 14351-1) with double (configuration 62 D) and triple (configuration 62) glazed window panes. The GPL variant has the largest weight per m2 in the 2-layer glazing product group. Since the frame/sash construction is alike across all variants in the product group, the parts that set the variants apart are primarily the window-operation components, such as hinges, handles and ventilation flaps. These components are to a high degree metal-based, and the worst-case product can thus be identified by the weight of products with similar size and glazing unit. The heavier the product, the larger the content of metal. Therefore, the GPL variant can be considered more representative as worst-case scenario for the whole roof windows group.", "lang": "en"}, {"value": "Die Hauptbestandteile des Standard-Holzdachfensters sind die Verglasungseinheit (hauptsächlich aus laminiertem und gehärtetem Glas), Holzrahmen/Flügel (aus Holz), Scharniere (aus Stahl) und Griffe/Lenker (aus Aluminium). Die Verpackung der Produkte besteht größtenteils aus Pappe samt Papiereinlage und verzinktem Stahl. Die Holzkomponenten (Flügel, Rahmen) werden intern in VELUX-Werken in Ungarn, Polen und Frankreich hergestellt. VELUX erhält gesägtes Kiefernholz (getrocknet) und verarbeitet es (Sägen, Schneiden etc.) zu Lamellen unterschiedlicher Qualität. Anschließend werden die Lamellen zusammengeklebt (laminiert) und zu Profilen verarbeitet (zuschneiden, beplanken, bohren etc.). Für die Verglasungseinheiten erhält VELUX die Verglasungseinheitenkomponenten von Lieferanten und produziert die endgültigen Verglasungseinheiten an Standorten in Ungarn, Dänemark, Frankreich und Deutschland. Nach ihrer Herstellung kommen die Verglasungen in den Fenstermontageprozess. Schließlich werden die Rahmen/Flügel, die Verglasungseinheit und die restlichen Komponenten (von Lieferanten geliefert) zu VELUX-Montagestandorten in Polen, Dänemark, Frankreich und Deutschland transportiert, wo sie zum endgültigen Fensterprodukt zusammengebaut werden. \nTechnische Daten: \nDie Leistungserklärung einschließlich relevanter technischer Spezifikationen und Testmethoden/Teststandards kann von der Website www.velux.com/ce heruntergeladen werden. \nDeklarierte Einheit: \nIn dieser EPD werden mehrere Produktdimensionen dargestellt, wie in der Produktbeschreibung angegeben. Die deklarierte Einheit ist 1 m2 Dachfenster aus Holz, berechnet auf der Grundlage der Größe 1,34 m x 1,40 m (UK08). Dies ist die verfügbare Größe, die der Referenzfenstergröße (1,23 m x 1,48 gemäß EN 14351-1) mit Doppelfenster (Konfiguration 62D) am nächsten kommt. und dreifach (Konfiguration 62) verglaste Fensterscheiben.", "lang": "de"}], "technologicalApplicability": [{"value": "VELUX wooden roof windows are used in renovation and new build. Either installed as a single window or in a combination of multiple windows.", "lang": "en"}, {"value": "VELUX Dachfenster aus Holz werden bei Renovierungen und Neubauten eingesetzt. Entweder als einzelnes Fenster oder in einer Kombination mehrerer Fenster installiert.", "lang": "de"}]}}, "modellingAndValidation": {"LCIMethodAndAllocation": {"typeOfDataSet": "EPD", "referenceToLCAMethodDetails": [{"shortDescription": [{"value": "Windows and doors .pdf", "lang": "en"}], "type": "source data set", "refObjectId": "a54d710a-ba43-4849-90db-2852c842b84e"}], "other": {"anies": [{"name": "subType", "value": "representative dataset"}]}}, "dataSourcesTreatmentAndRepresentativeness": {"referenceToDataSource": [{"shortDescription": [{"value": "GaBi Database (all versions)", "lang": "en"}], "type": "source data set", "refObjectId": "28d74cc0-db8b-4d7e-bc44-5f6d56ce0c4a"}, {"shortDescription": [{"value": "GaBi Database Edition 2021, CUP 2021.02", "lang": "en"}], "type": "source data set", "refObjectId": "90321ffe-9ebb-4946-886c-338efe6fbf26"}], "useAdviceForDataSet": [{"value": "Scope: \nThe EPD is a representative EPD covering VELUX wooden roof windows as specified in more detail in the product description. The products are manufactured by the VELUX Group at production sites in different locations in Europe for sale throughout Europe. The windows' production takes place in Poland, Denmark, France and Germany. \nSystem boundary: \nThe type of the EPD is \"cradle to gate - with options\" including the modules C1-C4 and D. The following life cycle phases were considered:\n\nProduct stage:\n\nA1 - Raw material supply: extraction and processing, production of the pre-products (e.g. laminated glass, sawn pine wood, metal/plastic components, sealants etc.) and sales packaging components (e.g., cardboard).\nA2 - Transport: Transport of pre-products and packaging components to the processing or assembly sites, as well as internal transportation of components between sites.\n\nA3 - Manufacturing: The wooden frames/sashes and glazing units are produced internally at VELUX production sites. Subsequently, the final production and assembly of the windows takes place, which involves activities such as shortening of profiles, drilling of holes, clamping and glueing, mounting of gaskets, brackets, panes etc.\n\nEnd of life stage:\n\nC1 - De-construction/demolition: deconstruction of the window with the use of an electric screwdriver and manual work.\n\nC2 - Transport: transport of window materials to Material Recovery Facilities (MRF) and then to incineration, landfill or recycling facilities. \n\nC3 - Waste processing: sorting of waste, recycling (metal and glass waste), incineration (plastic and wood waste) and landfill (metal, glass, wood and plastic waste).\n\nC4 - Disposal: disposal of all materials\n\nBenefits and loads beyond the system boundaries:\n\nD - Reuse, recovery and recycling potential: benefits from plastic and wood waste incineration processes and material recycling of metal and glass.\n\nFor the environmental impact, the use of green electricity was calculated taking into account the residual electricity mix for the remaining electricity. The proportion of the electricity demand covered by green electricity in the total electricity demand is 79.23 %.", "lang": "en"}, {"value": "Gültigkeitsbereich: \nLand oder Region, in der das deklarierte Produktsystem am Ende der Produktlebensdauer hergestellt, verwendet oder gehandhabt wird: Europa \nSystemgrenze: \nDer Typ der EPD ist „Cradle to Gate – mit Optionen“ inklusive der Module C1-C4 und D.", "lang": "de"}], "other": {"anies": [{"name": "referenceToOriginalEPD", "value": {"shortDescription": {"value": "VELUX wooden roof windows with glazing configuration 62 and 62D.pdf", "defaultValue": "VELUX wooden roof windows with glazing configuration 62 and 62D.pdf", "lstrings": [{"lang": "en", "value": "VELUX wooden roof windows with glazing configuration 62 and 62D.pdf"}]}, "type": "source data set", "uuid": {"uuid": "900bcf94-eff3-4d85-b300-9417d677d66c"}, "refObjectId": "900bcf94-eff3-4d85-b300-9417d677d66c", "resourceURLs": ["https://oekobaudat.de/OEKOBAU.DAT/resource/sources/900bcf94-eff3-4d85-b300-9417d677d66c/VELUX_wooden_roof_windows_with_glazing_configuration_62_and_62D_22230.pdf?version=00.02.000"]}}]}}, "validation": {"review": [{"referenceToNameOfReviewerAndInstitution": [{"shortDescription": [{"value": "Institut Bauen und Umwelt e. V.", "lang": "en"}], "type": "contact data set", "refObjectId": "d111dbec-b024-4be5-86c5-752d6eb2cf95", "uri": "../contacts/d111dbec-b024-4be5-86c5-752d6eb2cf95.xml"}], "type": "Accredited third party review"}]}, "complianceDeclarations": {"compliance": [{"referenceToComplianceSystem": {"shortDescription": [{"value": "DIN EN 15804+A2", "lang": "en"}], "type": "source data set", "refObjectId": "c0016b33-8cf7-415c-ac6e-deba0d21440d", "uri": "../sources/c0016b33-8cf7-415c-ac6e-deba0d21440d.xml"}}, {"referenceToComplianceSystem": {"shortDescription": [{"value": "ISO 14025", "lang": "en"}], "type": "source data set", "refObjectId": "4f2eb655-6e44-4874-a95a-e28f5442cd4d", "uri": "../sources/4f2eb655-6e44-4874-a95a-e28f5442cd4d.xml"}}]}}, "administrativeInformation": {"commissionerAndGoal": {"referenceToCommissioner": [{"shortDescription": [{"value": "VELUX Group", "lang": "en"}], "type": "contact data set", "refObjectId": "ab62e83b-7504-48ae-abdc-def53c14790d", "uri": "../contacts/ab62e83b-7504-48ae-abdc-def53c14790d.xml"}]}, "dataGenerator": {"referenceToPersonOrEntityGeneratingTheDataSet": [{"shortDescription": [{"value": "FORCE Technology", "lang": "en"}], "type": "contact data set", "refObjectId": "827dee6d-fd7f-4856-a4e8-0b3be8abfe6c", "uri": "../contacts/827dee6d-fd7f-4856-a4e8-0b3be8abfe6c.xml"}]}, "dataEntryBy": {"timeStamp": 1710115200000, "referenceToDataSetFormat": [{"shortDescription": [{"value": "ILCD Format", "lang": "en"}], "type": "source data set", "refObjectId": "a97a0155-0234-4b87-b4ce-a45da52f2a40", "uri": "../sources/a97a0155-0234-4b87-b4ce-a45da52f2a40.xml"}, {"shortDescription": [{"value": "EPD-Datenformaterweiterungen v1.2", "lang": "de"}, {"value": "EPD Data Format Extensions v1.2", "lang": "en"}], "type": "source data set", "refObjectId": "a29449fd-aa2f-4de8-b5d7-4b06b43c6fde", "uri": "../sources/a29449fd-aa2f-4de8-b5d7-4b06b43c6fde.xml"}]}, "publicationAndOwnership": {"dataSetVersion": "00.02.000", "referenceToRegistrationAuthority": {"shortDescription": [{"value": "Institut Bauen und Umwelt e. V.", "lang": "en"}], "type": "contact data set", "refObjectId": "d111dbec-b024-4be5-86c5-752d6eb2cf95", "uri": "../contacts/d111dbec-b024-4be5-86c5-752d6eb2cf95.xml"}, "registrationNumber": "EPD-VEL-20230511-CBJ1-EN", "referenceToOwnershipOfDataSet": {"shortDescription": [{"value": "VELUX Group", "lang": "en"}], "type": "contact data set", "refObjectId": "ab62e83b-7504-48ae-abdc-def53c14790d", "uri": "../contacts/ab62e83b-7504-48ae-abdc-def53c14790d.xml"}, "copyright": true, "licenseType": "Free of charge for all users and uses", "accessRestrictions": [{"value": "None", "lang": "en"}], "other": {"anies": [{"name": "referenceToPublisher", "value": {"shortDescription": [{"value": "Institut Bauen und Umwelt e. V.", "lang": "en"}], "type": "contact data set", "refObjectId": "d111dbec-b024-4be5-86c5-752d6eb2cf95", "uri": "../contacts/d111dbec-b024-4be5-86c5-752d6eb2cf95.xml"}}]}}}, "exchanges": {"exchange": [{"dataSetInternalID": 0, "referenceToFlowDataSet": {"shortDescription": [{"value": "VELUX standard wooden roof window (VELUX Holzdachfenster mit Verglasungskonfiguration 62 und 62D GPL-Variante)", "lang": "en"}], "type": "flow data set", "refObjectId": "f84f5517-2e50-fc92-b1ae-c24ade197386", "uri": "../flows/f84f5517-2e50-fc92-b1ae-c24ade197386.xml"}, "meanAmount": 1.0, "referencesToDataSource": {}, "referenceFlow": true, "resolvedFlowVersion": "00.04.000", "resultingflowAmount": 1.0, "flowProperties": [{"name": [{"lang": "de", "value": "Fläche"}, {"lang": "en", "value": "Area"}], "uuid": "93a60a56-a3c8-19da-a746-0800200c9a66", "referenceFlowProperty": true, "meanValue": 1.0, "referenceUnit": "qm", "unitGroupUUID": "c20a03d7-bd90-4569-bc94-66cfd364dfc8"}], "materialProperties": [{"name": "grammage", "value": "55.49", "unit": "kg/m^2", "unitDescription": "kilograms per square meter"}, {"name": "layer thickness", "value": "0.0377", "unit": "m", "unitDescription": "meters"}], "typeOfFlow": "Product flow", "classification": {"classHierarchy": "Komponenten von Fenstern und Vorhangfassaden / Fenster / Holzfenster", "name": "OEKOBAU.DAT"}}, {"dataSetInternalID": 1, "referenceToFlowDataSet": {"shortDescription": [{"value": "Renewable primary energy as energy carrier (PERE)", "lang": "en"}, {"value": "Erneuerbare Primärenergie als Energieträger (PERE)", "lang": "de"}], "type": "flow data set", "refObjectId": "20f32be5-0398-4288-9b6d-accddd195317", "uri": "../flows/20f32be5-0398-4288-9b6d-accddd195317.xml"}, "exchange direction": "INPUT", "other": {"anies": [{"name": "referenceToUnitGroupDataSet", "value": {"shortDescription": [{"value": "MJ", "lang": "en"}], "type": "unit group data set", "refObjectId": "93a60a57-a3c8-11da-a746-0800200c9a66", "uri": "../unitgroups/93a60a57-a3c8-11da-a746-0800200c9a66.xml"}}, {"value": "560.209095305123", "module": "A1"}, {"value": "0.353197868439763", "module": "A2"}, {"value": "429.828540930335", "module": "A3"}, {"value": "0.00420815665226522", "module": "C1"}, {"value": "2.37719656083686", "module": "C2"}, {"value": "1.01899739457521", "module": "C3"}, {"value": "0.643408411869302", "module": "C4"}, {"value": "-75.7584056997846", "module": "D"}]}, "resolvedFlowVersion": "38.00.000", "flowProperties": [], "typeOfFlow": "Other flow", "classification": {"classHierarchy": "Quantities", "name": "GaBiCategories"}}, {"dataSetInternalID": 2, "referenceToFlowDataSet": {"shortDescription": [{"value": "Renewable primary energy resources as material utilization (PERM)", "lang": "en"}, {"value": "Erneuerbare Primärenergie zur stofflichen Nutzung (PERM)", "lang": "de"}], "type": "flow data set", "refObjectId": "fb3ec0de-548d-4508-aea5-00b73bf6f702", "uri": "../flows/fb3ec0de-548d-4508-aea5-00b73bf6f702.xml"}, "exchange direction": "INPUT", "other": {"anies": [{"name": "referenceToUnitGroupDataSet", "value": {"shortDescription": [{"value": "MJ", "lang": "en"}], "type": "unit group data set", "refObjectId": "93a60a57-a3c8-11da-a746-0800200c9a66", "uri": "../unitgroups/93a60a57-a3c8-11da-a746-0800200c9a66.xml"}}, {"value": "0.0834168609865471", "module": "A1"}, {"value": "0", "module": "A2"}, {"value": "0", "module": "A3"}, {"value": "0", "module": "C1"}, {"value": "0", "module": "C2"}, {"value": "0", "module": "C3"}, {"value": "0", "module": "C4"}, {"value": "0", "module": "D"}]}, "resolvedFlowVersion": "38.00.000", "flowProperties": [], "typeOfFlow": "Other flow", "classification": {"classHierarchy": "Quantities", "name": "GaBiCategories"}}, {"dataSetInternalID": 3, "referenceToFlowDataSet": {"shortDescription": [{"value": "Total use of renewable primary energy resources (PERT)", "lang": "en"}, {"value": "Total erneuerbare Primärenergie (PERT)", "lang": "de"}], "type": "flow data set", "refObjectId": "53f97275-fa8a-4cdd-9024-65936002acd0", "uri": "../flows/53f97275-fa8a-4cdd-9024-65936002acd0.xml"}, "exchange direction": "INPUT", "other": {"anies": [{"name": "referenceToUnitGroupDataSet", "value": {"shortDescription": [{"value": "MJ", "lang": "en"}], "type": "unit group data set", "refObjectId": "93a60a57-a3c8-11da-a746-0800200c9a66", "uri": "../unitgroups/93a60a57-a3c8-11da-a746-0800200c9a66.xml"}}, {"value": "560.309597547276", "module": "A1"}, {"value": "0.353197868439763", "module": "A2"}, {"value": "429.828540930335", "module": "A3"}, {"value": "0.00420815665226522", "module": "C1"}, {"value": "2.37719656083686", "module": "C2"}, {"value": "1.01899739457521", "module": "C3"}, {"value": "0.643408411869302", "module": "C4"}, {"value": "-75.7584056997846", "module": "D"}]}, "resolvedFlowVersion": "38.00.000", "flowProperties": [], "typeOfFlow": "Other flow", "classification": {"classHierarchy": "Quantities / Environmental quantities / EPD EN 15804 / LCI indicators", "name": "GaBiCategories"}}, {"dataSetInternalID": 4, "referenceToFlowDataSet": {"shortDescription": [{"value": "Non renewable primary energy as energy carrier (PENRE)", "lang": "en"}, {"value": "Nicht-erneuerbare Primärenergie als Energieträger (PENRE)", "lang": "de"}], "type": "flow data set", "refObjectId": "ac857178-2b45-46ec-892a-a9a4332f0372", "uri": "../flows/ac857178-2b45-46ec-892a-a9a4332f0372.xml"}, "exchange direction": "INPUT", "other": {"anies": [{"name": "referenceToUnitGroupDataSet", "value": {"shortDescription": [{"value": "MJ", "lang": "en"}], "type": "unit group data set", "refObjectId": "93a60a57-a3c8-11da-a746-0800200c9a66", "uri": "../unitgroups/93a60a57-a3c8-11da-a746-0800200c9a66.xml"}}, {"value": "1719.66705303887", "module": "A1"}, {"value": "6.25988437835041", "module": "A2"}, {"value": "226.61410686039", "module": "A3"}, {"value": "0.0408509850670676", "module": "C1"}, {"value": "41.4624593302665", "module": "C2"}, {"value": "101.56942841209", "module": "C3"}, {"value": "5.03603931452981", "module": "C4"}, {"value": "-450.345119712563", "module": "D"}]}, "resolvedFlowVersion": "38.00.000", "flowProperties": [], "typeOfFlow": "Other flow", "classification": {"classHierarchy": "Quantities", "name": "GaBiCategories"}}, {"dataSetInternalID": 5, "referenceToFlowDataSet": {"shortDescription": [{"value": "Non renewable primary energy as material utilization (PENRM)", "lang": "en"}, {"value": "Nicht-erneuerbare Primärenergie zur stofflichen Nutzung (PENRM)", "lang": "de"}], "type": "flow data set", "refObjectId": "1421caa0-679d-4bf4-b282-0eb850ccae27", "uri": "../flows/1421caa0-679d-4bf4-b282-0eb850ccae27.xml"}, "exchange direction": "INPUT", "other": {"anies": [{"name": "referenceToUnitGroupDataSet", "value": {"shortDescription": [{"value": "MJ", "lang": "en"}], "type": "unit group data set", "refObjectId": "93a60a57-a3c8-11da-a746-0800200c9a66", "uri": "../unitgroups/93a60a57-a3c8-11da-a746-0800200c9a66.xml"}}, {"value": "132.0593861934", "module": "A1"}, {"value": "0", "module": "A2"}, {"value": "-0.50855832420595", "module": "A3"}, {"value": "0", "module": "C1"}, {"value": "0", "module": "C2"}, {"value": "-96.2061295", "module": "C3"}, {"value": "0", "module": "C4"}, {"value": "0", "module": "D"}]}, "resolvedFlowVersion": "38.00.000", "flowProperties": [], "typeOfFlow": "Other flow", "classification": {"classHierarchy": "Quantities", "name": "GaBiCategories"}}, {"dataSetInternalID": 6, "referenceToFlowDataSet": {"shortDescription": [{"value": "Total use of non renewable primary energy resources (PENRT)", "lang": "en"}, {"value": "Total nicht erneuerbare Primärenergie (PENRT)", "lang": "de"}], "type": "flow data set", "refObjectId": "06159210-646b-4c8d-8583-da9b3b95a6c1", "uri": "../flows/06159210-646b-4c8d-8583-da9b3b95a6c1.xml"}, "exchange direction": "INPUT", "other": {"anies": [{"name": "referenceToUnitGroupDataSet", "value": {"shortDescription": [{"value": "MJ", "lang": "en"}], "type": "unit group data set", "refObjectId": "93a60a57-a3c8-11da-a746-0800200c9a66", "uri": "../unitgroups/93a60a57-a3c8-11da-a746-0800200c9a66.xml"}}, {"value": "1851.93158887455", "module": "A1"}, {"value": "6.25988437835045", "module": "A2"}, {"value": "226.105886448339", "module": "A3"}, {"value": "0.0408509850670681", "module": "C1"}, {"value": "41.4624593302668", "module": "C2"}, {"value": "5.36329105399693", "module": "C3"}, {"value": "5.0360393145299", "module": "C4"}, {"value": "-450.34511971257", "module": "D"}]}, "resolvedFlowVersion": "38.00.000", "flowProperties": [], "typeOfFlow": "Other flow", "classification": {"classHierarchy": "Quantities / Environmental quantities / EPD EN 15804 / LCI indicators", "name": "GaBiCategories"}}, {"dataSetInternalID": 7, "referenceToFlowDataSet": {"shortDescription": [{"value": "Use of secondary material (SM)", "lang": "en"}, {"value": "Einsatz von Sekundärstoffen (SM)", "lang": "de"}], "type": "flow data set", "refObjectId": "c6a1f35f-2d09-4f54-8dfb-97e502e1ce92", "uri": "../flows/c6a1f35f-2d09-4f54-8dfb-97e502e1ce92.xml"}, "exchange direction": "INPUT", "other": {"anies": [{"name": "referenceToUnitGroupDataSet", "value": {"shortDescription": [{"value": "kg", "lang": "en"}], "type": "unit group data set", "refObjectId": "ad38d542-3fe9-439d-9b95-2f5f7752acaf", "uri": "../unitgroups/ad38d542-3fe9-439d-9b95-2f5f7752acaf.xml"}}, {"value": "3.81598756959538", "module": "A1"}, {"value": "0", "module": "A2"}, {"value": "0", "module": "A3"}, {"value": "0", "module": "C1"}, {"value": "0", "module": "C2"}, {"value": "0", "module": "C3"}, {"value": "0", "module": "C4"}, {"value": "0", "module": "D"}]}, "resolvedFlowVersion": "38.00.000", "flowProperties": [], "typeOfFlow": "Other flow", "classification": {"classHierarchy": "Quantities / Environmental quantities / EPD EN 15804 / LCI indicators", "name": "GaBiCategories"}}, {"dataSetInternalID": 8, "referenceToFlowDataSet": {"shortDescription": [{"value": "Use of renewable secondary fuels (RSF)", "lang": "en"}, {"value": "Erneuerbare Sekundärbrennstoffe (RSF)", "lang": "de"}], "type": "flow data set", "refObjectId": "64333088-a55f-4aa2-9a31-c10b07816787", "uri": "../flows/64333088-a55f-4aa2-9a31-c10b07816787.xml"}, "exchange direction": "INPUT", "other": {"anies": [{"name": "referenceToUnitGroupDataSet", "value": {"shortDescription": [{"value": "MJ", "lang": "en"}], "type": "unit group data set", "refObjectId": "93a60a57-a3c8-11da-a746-0800200c9a66", "uri": "../unitgroups/93a60a57-a3c8-11da-a746-0800200c9a66.xml"}}, {"value": "0", "module": "A1"}, {"value": "0", "module": "A2"}, {"value": "0", "module": "A3"}, {"value": "0", "module": "C1"}, {"value": "0", "module": "C2"}, {"value": "0", "module": "C3"}, {"value": "0", "module": "C4"}, {"value": "0", "module": "D"}]}, "resolvedFlowVersion": "38.00.000", "flowProperties": [], "typeOfFlow": "Other flow", "classification": {"classHierarchy": "Quantities / Environmental quantities / EPD EN 15804 / LCI indicators", "name": "GaBiCategories"}}, {"dataSetInternalID": 9, "referenceToFlowDataSet": {"shortDescription": [{"value": "Use of non renewable secondary fuels (NRSF)", "lang": "en"}, {"value": "Nicht erneuerbare Sekundärbrennstoffe (NRSF)", "lang": "de"}], "type": "flow data set", "refObjectId": "89def144-d39a-4287-b86f-efde453ddcb2", "uri": "../flows/89def144-d39a-4287-b86f-efde453ddcb2.xml"}, "exchange direction": "INPUT", "other": {"anies": [{"name": "referenceToUnitGroupDataSet", "value": {"shortDescription": [{"value": "MJ", "lang": "en"}], "type": "unit group data set", "refObjectId": "93a60a57-a3c8-11da-a746-0800200c9a66", "uri": "../unitgroups/93a60a57-a3c8-11da-a746-0800200c9a66.xml"}}, {"value": "0", "module": "A1"}, {"value": "0", "module": "A2"}, {"value": "0", "module": "A3"}, {"value": "0", "module": "C1"}, {"value": "0", "module": "C2"}, {"value": "0", "module": "C3"}, {"value": "0", "module": "C4"}, {"value": "0", "module": "D"}]}, "resolvedFlowVersion": "38.00.000", "flowProperties": [], "typeOfFlow": "Other flow", "classification": {"classHierarchy": "Quantities / Environmental quantities / EPD EN 15804 / LCI indicators", "name": "GaBiCategories"}}, {"dataSetInternalID": 10, "referenceToFlowDataSet": {"shortDescription": [{"value": "Use of net fresh water (FW)", "lang": "en"}, {"value": "Einsatz von Süßwasserressourcen (FW)", "lang": "de"}], "type": "flow data set", "refObjectId": "3cf952c8-f3a4-461d-8c96-96456ca62246", "uri": "../flows/3cf952c8-f3a4-461d-8c96-96456ca62246.xml"}, "exchange direction": "INPUT", "other": {"anies": [{"name": "referenceToUnitGroupDataSet", "value": {"shortDescription": [{"value": "m^3", "lang": "en"}], "type": "unit group data set", "refObjectId": "cd950537-0a98-4044-9ba7-9f9a68d0a504", "uri": "../unitgroups/cd950537-0a98-4044-9ba7-9f9a68d0a504.xml"}}, {"value": "0.572771336678102", "module": "A1"}, {"value": "0.000404701237694441", "module": "A2"}, {"value": "0.0669558978061131", "module": "A3"}, {"value": "9.19864857472407E-06", "module": "C1"}, {"value": "0.00272265987865747", "module": "C2"}, {"value": "0.0488789498955614", "module": "C3"}, {"value": "0.00119379717276416", "module": "C4"}, {"value": "-0.180874067493988", "module": "D"}]}, "resolvedFlowVersion": "38.00.000", "flowProperties": [], "typeOfFlow": "Other flow", "classification": {"classHierarchy": "Quantities / Environmental quantities / EPD EN 15804 / LCI indicators", "name": "GaBiCategories"}}, {"dataSetInternalID": 11, "referenceToFlowDataSet": {"shortDescription": [{"value": "Hazardous waste disposed (HWD)", "lang": "en"}, {"value": "Gefährlicher Abfall zur Deponie (HWD)", "lang": "de"}], "type": "flow data set", "refObjectId": "430f9e0f-59b2-46a0-8e0d-55e0e84948fc", "uri": "../flows/430f9e0f-59b2-46a0-8e0d-55e0e84948fc.xml"}, "exchange direction": "OUTPUT", "other": {"anies": [{"name": "referenceToUnitGroupDataSet", "value": {"shortDescription": [{"value": "kg", "lang": "en"}], "type": "unit group data set", "refObjectId": "ad38d542-3fe9-439d-9b95-2f5f7752acaf", "uri": "../unitgroups/ad38d542-3fe9-439d-9b95-2f5f7752acaf.xml"}}, {"value": "0.00324940292719574", "module": "A1"}, {"value": "3.25091013229289E-10", "module": "A2"}, {"value": "1.26057146303714E-06", "module": "A3"}, {"value": "4.91239086190618E-12", "module": "C1"}, {"value": "2.18474624551329E-09", "module": "C2"}, {"value": "1.08366442240402E-09", "module": "C3"}, {"value": "5.75426008005187E-10", "module": "C4"}, {"value": "-4.53840730774836E-08", "module": "D"}]}, "resolvedFlowVersion": "38.00.000", "flowProperties": [], "typeOfFlow": "Other flow", "classification": {"classHierarchy": "Quantities / Environmental quantities / EPD EN 15804 / LCI indicators", "name": "GaBiCategories"}}, {"dataSetInternalID": 12, "referenceToFlowDataSet": {"shortDescription": [{"value": "Non hazardous waste disposed (NHWD)", "lang": "en"}, {"value": "Entsorgter nicht gefährlicher Abfall (NHWD)", "lang": "de"}], "type": "flow data set", "refObjectId": "b29ef66b-e286-4afa-949f-62f1a7b4d7fa", "uri": "../flows/b29ef66b-e286-4afa-949f-62f1a7b4d7fa.xml"}, "exchange direction": "OUTPUT", "other": {"anies": [{"name": "referenceToUnitGroupDataSet", "value": {"shortDescription": [{"value": "kg", "lang": "en"}], "type": "unit group data set", "refObjectId": "ad38d542-3fe9-439d-9b95-2f5f7752acaf", "uri": "../unitgroups/ad38d542-3fe9-439d-9b95-2f5f7752acaf.xml"}}, {"value": "8.48826868236762", "module": "A1"}, {"value": "0.000976115838820809", "module": "A2"}, {"value": "0.346847813418456", "module": "A3"}, {"value": "7.67606509628827E-06", "module": "C1"}, {"value": "0.00650496349220989", "module": "C2"}, {"value": "0.962049810301922", "module": "C3"}, {"value": "22.7227634536422", "module": "C4"}, {"value": "-3.39066424859372", "module": "D"}]}, "resolvedFlowVersion": "38.00.000", "flowProperties": [], "typeOfFlow": "Other flow", "classification": {"classHierarchy": "Quantities / Environmental quantities / EPD EN 15804 / LCI indicators", "name": "GaBiCategories"}}, {"dataSetInternalID": 13, "referenceToFlowDataSet": {"shortDescription": [{"value": "Radioactive waste disposed (RWD)", "lang": "en"}, {"value": "Entsorgter radioaktiver Abfall (RWD)", "lang": "de"}], "type": "flow data set", "refObjectId": "3449546e-52ad-4b39-b809-9fb77cea8ff6", "uri": "../flows/3449546e-52ad-4b39-b809-9fb77cea8ff6.xml"}, "exchange direction": "OUTPUT", "other": {"anies": [{"name": "referenceToUnitGroupDataSet", "value": {"shortDescription": [{"value": "kg", "lang": "en"}], "type": "unit group data set", "refObjectId": "ad38d542-3fe9-439d-9b95-2f5f7752acaf", "uri": "../unitgroups/ad38d542-3fe9-439d-9b95-2f5f7752acaf.xml"}}, {"value": "0.0437616303742368", "module": "A1"}, {"value": "1.1280664927527E-05", "module": "A2"}, {"value": "0.0108821798996243", "module": "A3"}, {"value": "6.61046291154375E-06", "module": "C1"}, {"value": "7.52098325500536E-05", "module": "C2"}, {"value": "0.000260457178550171", "module": "C3"}, {"value": "5.33912666856923E-05", "module": "C4"}, {"value": "-0.0170730341400518", "module": "D"}]}, "resolvedFlowVersion": "38.00.000", "flowProperties": [], "typeOfFlow": "Other flow", "classification": {"classHierarchy": "Quantities / Environmental quantities / EPD EN 15804 / LCI indicators", "name": "GaBiCategories"}}, {"dataSetInternalID": 14, "referenceToFlowDataSet": {"shortDescription": [{"value": "Components for re-use (CRU)", "lang": "en"}, {"value": "Komponenten für die Wiederverwendung (CRU)", "lang": "de"}], "type": "flow data set", "refObjectId": "a2b32f97-3fc7-4af2-b209-525bc6426f33", "uri": "../flows/a2b32f97-3fc7-4af2-b209-525bc6426f33.xml"}, "exchange direction": "OUTPUT", "other": {"anies": [{"name": "referenceToUnitGroupDataSet", "value": {"shortDescription": [{"value": "kg", "lang": "en"}], "type": "unit group data set", "refObjectId": "ad38d542-3fe9-439d-9b95-2f5f7752acaf", "uri": "../unitgroups/ad38d542-3fe9-439d-9b95-2f5f7752acaf.xml"}}, {"value": "0", "module": "A1"}, {"value": "0", "module": "A2"}, {"value": "0", "module": "A3"}, {"value": "0", "module": "C1"}, {"value": "0", "module": "C2"}, {"value": "0", "module": "C3"}, {"value": "0", "module": "C4"}, {"value": "0", "module": "D"}]}, "resolvedFlowVersion": "38.00.000", "flowProperties": [], "typeOfFlow": "Other flow", "classification": {"classHierarchy": "Quantities / Environmental quantities / EPD EN 15804 / LCI indicators", "name": "GaBiCategories"}}, {"dataSetInternalID": 15, "referenceToFlowDataSet": {"shortDescription": [{"value": "Materials for recycling (MFR)", "lang": "en"}, {"value": "Stoffe zum Recycling (MFR)", "lang": "de"}], "type": "flow data set", "refObjectId": "d7fe48a5-4103-49c8-9aae-b0b5dfdbd6ae", "uri": "../flows/d7fe48a5-4103-49c8-9aae-b0b5dfdbd6ae.xml"}, "exchange direction": "OUTPUT", "other": {"anies": [{"name": "referenceToUnitGroupDataSet", "value": {"shortDescription": [{"value": "kg", "lang": "en"}], "type": "unit group data set", "refObjectId": "ad38d542-3fe9-439d-9b95-2f5f7752acaf", "uri": "../unitgroups/ad38d542-3fe9-439d-9b95-2f5f7752acaf.xml"}}, {"value": "0.0176883946188341", "module": "A1"}, {"value": "0", "module": "A2"}, {"value": "17.518862639569", "module": "A3"}, {"value": "0", "module": "C1"}, {"value": "0", "module": "C2"}, {"value": "18.352815", "module": "C3"}, {"value": "0", "module": "C4"}, {"value": "0", "module": "D"}]}, "resolvedFlowVersion": "38.00.000", "flowProperties": [], "typeOfFlow": "Other flow", "classification": {"classHierarchy": "Quantities / Environmental quantities / EPD EN 15804 / LCI indicators", "name": "GaBiCategories"}}, {"dataSetInternalID": 16, "referenceToFlowDataSet": {"shortDescription": [{"value": "Materials for energy recovery (MER)", "lang": "en"}, {"value": "Stoffe für die Energierückgewinnung (MER)", "lang": "de"}], "type": "flow data set", "refObjectId": "59a9181c-3aaf-46ee-8b13-2b3723b6e447", "uri": "../flows/59a9181c-3aaf-46ee-8b13-2b3723b6e447.xml"}, "exchange direction": "OUTPUT", "other": {"anies": [{"name": "referenceToUnitGroupDataSet", "value": {"shortDescription": [{"value": "kg", "lang": "en"}], "type": "unit group data set", "refObjectId": "ad38d542-3fe9-439d-9b95-2f5f7752acaf", "uri": "../unitgroups/ad38d542-3fe9-439d-9b95-2f5f7752acaf.xml"}}, {"value": "0", "module": "A1"}, {"value": "0", "module": "A2"}, {"value": "0", "module": "A3"}, {"value": "0", "module": "C1"}, {"value": "0", "module": "C2"}, {"value": "10.437935", "module": "C3"}, {"value": "0", "module": "C4"}, {"value": "0", "module": "D"}]}, "resolvedFlowVersion": "38.00.000", "flowProperties": [], "typeOfFlow": "Other flow", "classification": {"classHierarchy": "Quantities / Environmental quantities / EPD EN 15804 / LCI indicators", "name": "GaBiCategories"}}, {"dataSetInternalID": 17, "referenceToFlowDataSet": {"shortDescription": [{"value": "Exported electrical energy (EEE)", "lang": "en"}, {"value": "Exportierte elektrische Energie (EEE)", "lang": "de"}], "type": "flow data set", "refObjectId": "4da0c987-2b76-40d6-9e9e-82a017aaaf29", "uri": "../flows/4da0c987-2b76-40d6-9e9e-82a017aaaf29.xml"}, "exchange direction": "OUTPUT", "other": {"anies": [{"name": "referenceToUnitGroupDataSet", "value": {"shortDescription": [{"value": "MJ", "lang": "en"}], "type": "unit group data set", "refObjectId": "93a60a57-a3c8-11da-a746-0800200c9a66", "uri": "../unitgroups/93a60a57-a3c8-11da-a746-0800200c9a66.xml"}}, {"value": "0.035125533632287", "module": "A1"}, {"value": "0", "module": "A2"}, {"value": "0", "module": "A3"}, {"value": "0", "module": "C1"}, {"value": "0", "module": "C2"}, {"value": "32.8495717981645", "module": "C3"}, {"value": "0", "module": "C4"}, {"value": "0", "module": "D"}]}, "resolvedFlowVersion": "38.00.000", "flowProperties": [], "typeOfFlow": "Other flow", "classification": {"classHierarchy": "Quantities / Environmental quantities / EPD EN 15804 / LCI indicators", "name": "GaBiCategories"}}, {"dataSetInternalID": 18, "referenceToFlowDataSet": {"shortDescription": [{"value": "Exported thermal energy (EET)", "lang": "en"}, {"value": "Exportierte thermische Energie (EET)", "lang": "de"}], "type": "flow data set", "refObjectId": "98daf38a-7a79-46d3-9a37-2b7bd0955810", "uri": "../flows/98daf38a-7a79-46d3-9a37-2b7bd0955810.xml"}, "exchange direction": "OUTPUT", "other": {"anies": [{"name": "referenceToUnitGroupDataSet", "value": {"shortDescription": [{"value": "MJ", "lang": "en"}], "type": "unit group data set", "refObjectId": "93a60a57-a3c8-11da-a746-0800200c9a66", "uri": "../unitgroups/93a60a57-a3c8-11da-a746-0800200c9a66.xml"}}, {"value": "0.0512561434977578", "module": "A1"}, {"value": "0", "module": "A2"}, {"value": "0", "module": "A3"}, {"value": "0", "module": "C1"}, {"value": "0", "module": "C2"}, {"value": "59.7618146761373", "module": "C3"}, {"value": "0", "module": "C4"}, {"value": "0", "module": "D"}]}, "resolvedFlowVersion": "38.00.000", "flowProperties": [], "typeOfFlow": "Other flow", "classification": {"classHierarchy": "Quantities / Environmental quantities / EPD EN 15804 / LCI indicators", "name": "GaBiCategories"}}]}, "LCIAResults": {"LCIAResult": [{"referenceToLCIAMethodDataSet": {"shortDescription": [{"value": "Global Warming Potential total (GWP-total)", "lang": "en"}, {"value": "Globales Erwärmungspotenzial total (GWP-total)", "lang": "de"}], "type": "LCIA method data set", "refObjectId": "6a37f984-a4b3-458a-a20a-64418c145fa2", "uri": "../lciamethods/6a37f984-a4b3-458a-a20a-64418c145fa2.xml"}, "other": {"anies": [{"name": "referenceToUnitGroupDataSet", "value": {"shortDescription": [{"value": "kg CO_(2) eq", "lang": "en"}], "type": "unit group data set", "refObjectId": "1ebf3012-d0db-4de2-aefd-ef30cedb0be1", "uri": "../unitgroups/1ebf3012-d0db-4de2-aefd-ef30cedb0be1.xml"}}, {"value": "108.294139897777", "module": "A1"}, {"value": "0.472763472473999", "module": "A2"}, {"value": "25.7181973239109", "module": "A3"}, {"value": "0.00197256475594537", "module": "C1"}, {"value": "3.12603509805706", "module": "C2"}, {"value": "18.6713795484759", "module": "C3"}, {"value": "1.91", "module": "C4"}, {"value": "-37.0652939970459", "module": "D"}]}}, {"referenceToLCIAMethodDataSet": {"shortDescription": [{"value": "Global Warming Potential fossil fuels (GWP-fossil)", "lang": "en"}, {"value": "Globales Erwärmungspotenzial fossil (GWP-fossil)", "lang": "de"}], "type": "LCIA method data set", "refObjectId": "5f635281-343e-44fb-83df-1971b155e6b6", "uri": "../lciamethods/5f635281-343e-44fb-83df-1971b155e6b6.xml"}, "other": {"anies": [{"name": "referenceToUnitGroupDataSet", "value": {"shortDescription": [{"value": "kg CO_(2) eq", "lang": "en"}], "type": "unit group data set", "refObjectId": "1ebf3012-d0db-4de2-aefd-ef30cedb0be1", "uri": "../unitgroups/1ebf3012-d0db-4de2-aefd-ef30cedb0be1.xml"}}, {"value": "136.123198725395", "module": "A1"}, {"value": "0.469537511864936", "module": "A2"}, {"value": "15.0635457584379", "module": "A3"}, {"value": "0.0019711222585743", "module": "C1"}, {"value": "3.06763626738595", "module": "C2"}, {"value": "5.97873263733917", "module": "C3"}, {"value": "0.377510997579113", "module": "C4"}, {"value": "-37.0023721532117", "module": "D"}]}}, {"referenceToLCIAMethodDataSet": {"shortDescription": [{"value": "Global Warming Potential biogenic (GWP-biogenic)", "lang": "en"}, {"value": "Globales Erwärmungspotenzial biogen (GWP-biogenic)", "lang": "de"}], "type": "LCIA method data set", "refObjectId": "2356e1ab-0185-4db5-86e5-16de51c7485c", "uri": "../lciamethods/2356e1ab-0185-4db5-86e5-16de51c7485c.xml"}, "other": {"anies": [{"name": "referenceToUnitGroupDataSet", "value": {"shortDescription": [{"value": "kg CO_(2) eq", "lang": "en"}], "type": "unit group data set", "refObjectId": "1ebf3012-d0db-4de2-aefd-ef30cedb0be1", "uri": "../unitgroups/1ebf3012-d0db-4de2-aefd-ef30cedb0be1.xml"}}, {"value": "-28.0561178917383", "module": "A1"}, {"value": "-0.000537035101812629", "module": "A2"}, {"value": "10.6283264230811", "module": "A3"}, {"value": "1.10491593051375E-06", "module": "C1"}, {"value": "0.0330471618788666", "module": "C2"}, {"value": "12.6920194862481", "module": "C3"}, {"value": "1.53", "module": "C4"}, {"value": "-0.0516664001719831", "module": "D"}]}}, {"referenceToLCIAMethodDataSet": {"shortDescription": [{"value": "Global Warming Potential luluc (GWP-luluc)", "lang": "en"}, {"value": "Globales Erwärmungspotenzial luluc (GWP-luluc)", "lang": "de"}], "type": "LCIA method data set", "refObjectId": "4331bbdb-978a-490d-8707-eeb047f01a55", "uri": "../lciamethods/4331bbdb-978a-490d-8707-eeb047f01a55.xml"}, "other": {"anies": [{"name": "referenceToUnitGroupDataSet", "value": {"shortDescription": [{"value": "kg CO_(2) eq", "lang": "en"}], "type": "unit group data set", "refObjectId": "1ebf3012-d0db-4de2-aefd-ef30cedb0be1", "uri": "../unitgroups/1ebf3012-d0db-4de2-aefd-ef30cedb0be1.xml"}}, {"value": "0.0894714946131943", "module": "A1"}, {"value": "0.00376299571087562", "module": "A2"}, {"value": "0.0263251423920022", "module": "A3"}, {"value": "3.37581440556109E-07", "module": "C1"}, {"value": "0.0253516687922501", "module": "C2"}, {"value": "0.000627424888611966", "module": "C3"}, {"value": "0.00102390523395931", "module": "C4"}, {"value": "-0.0112554436622082", "module": "D"}]}}, {"referenceToLCIAMethodDataSet": {"shortDescription": [{"value": "Depletion potential of the stratospheric ozone layer (ODP)", "lang": "en"}, {"value": "Abbau Potential der stratosphärischen Ozonschicht (ODP)", "lang": "de"}], "type": "LCIA method data set", "refObjectId": "b5c629d6-def3-11e6-bf01-fe55135034f3", "uri": "../lciamethods/b5c629d6-def3-11e6-bf01-fe55135034f3.xml"}, "other": {"anies": [{"name": "referenceToUnitGroupDataSet", "value": {"shortDescription": [{"value": "kg CFC11 eq", "lang": "en"}], "type": "unit group data set", "refObjectId": "d9e957c9-7309-4474-bf3a-7777df6c4e5b", "uri": "../unitgroups/d9e957c9-7309-4474-bf3a-7777df6c4e5b.xml"}}, {"value": "1.16813301265759E-06", "module": "A1"}, {"value": "9.1783465052477E-17", "module": "A2"}, {"value": "1.44709944037671E-09", "module": "A3"}, {"value": "2.21770126126117E-17", "module": "C1"}, {"value": "6.12338869340224E-16", "module": "C2"}, {"value": "-9.08412363251436E-09", "module": "C3"}, {"value": "1.40307288523622E-15", "module": "C4"}, {"value": "-5.77717649533567E-14", "module": "D"}]}}, {"referenceToLCIAMethodDataSet": {"shortDescription": [{"value": "Acidification potential of land and water (AP)", "lang": "en"}, {"value": "Versauerungspotenzial von Boden und Wasser (AP)", "lang": "de"}], "type": "LCIA method data set", "refObjectId": "b5c611c6-def3-11e6-bf01-fe55135034f3", "uri": "../lciamethods/b5c611c6-def3-11e6-bf01-fe55135034f3.xml"}, "other": {"anies": [{"name": "referenceToUnitGroupDataSet", "value": {"shortDescription": [{"value": "mol H^(+) eq", "lang": "en"}], "type": "unit group data set", "refObjectId": "42e089ac-92bf-4bf2-8ca1-5fc40d18f2ed", "uri": "../unitgroups/42e089ac-92bf-4bf2-8ca1-5fc40d18f2ed.xml"}}, {"value": "0.613120763137287", "module": "A1"}, {"value": "0.000716161010807074", "module": "A2"}, {"value": "0.0429681718974007", "module": "A3"}, {"value": "3.18435349310474E-06", "module": "C1"}, {"value": "0.01866554068583", "module": "C2"}, {"value": "0.00535164584997662", "module": "C3"}, {"value": "0.00260879085085186", "module": "C4"}, {"value": "-0.138305573407294", "module": "D"}]}}, {"referenceToLCIAMethodDataSet": {"shortDescription": [{"value": "Eutrophication potential aquatic freshwater (EP-freshwater)", "lang": "en"}, {"value": "Eutrophierungspotenzial Süßwasser (EP-freshwater)", "lang": "de"}], "type": "LCIA method data set", "refObjectId": "b53ec18f-7377-4ad3-86eb-cc3f4f276b2b", "uri": "../lciamethods/b53ec18f-7377-4ad3-86eb-cc3f4f276b2b.xml"}, "other": {"anies": [{"name": "referenceToUnitGroupDataSet", "value": {"shortDescription": [{"value": "kg P eq", "lang": "en"}], "type": "unit group data set", "refObjectId": "0429039d-a61d-4590-ba67-aa4a20a810a1", "uri": "../unitgroups/0429039d-a61d-4590-ba67-aa4a20a810a1.xml"}}, {"value": "0.0048118159913422", "module": "A1"}, {"value": "1.36960938531169E-06", "module": "A2"}, {"value": "0.000143832328304893", "module": "A3"}, {"value": "7.92200616277336E-10", "module": "C1"}, {"value": "9.21443817130362E-06", "module": "C2"}, {"value": "-2.08674747229934E-05", "module": "C3"}, {"value": "3.55312425458262E-06", "module": "C4"}, {"value": "-1.96893816601126E-05", "module": "D"}]}}, {"referenceToLCIAMethodDataSet": {"shortDescription": [{"value": "Eutrophication potential aquatic marine (EP-marine)", "lang": "en"}, {"value": "Eutrophierungspotenzial Salzwasser (EP-marine)", "lang": "de"}], "type": "LCIA method data set", "refObjectId": "b5c619fa-def3-11e6-bf01-fe55135034f3", "uri": "../lciamethods/b5c619fa-def3-11e6-bf01-fe55135034f3.xml"}, "other": {"anies": [{"name": "referenceToUnitGroupDataSet", "value": {"shortDescription": [{"value": "kg N eq", "lang": "en"}], "type": "unit group data set", "refObjectId": "d05bb823-ecdf-4686-8c40-bf1d9257859f", "uri": "../unitgroups/d05bb823-ecdf-4686-8c40-bf1d9257859f.xml"}}, {"value": "0.129312412013817", "module": "A1"}, {"value": "0.000241046747026222", "module": "A2"}, {"value": "0.016951905529285", "module": "A3"}, {"value": "8.42624838426716E-07", "module": "C1"}, {"value": "0.00912385256604872", "module": "C2"}, {"value": "0.00230684116282296", "module": "C3"}, {"value": "0.00070543918900958", "module": "C4"}, {"value": "-0.0298518207068079", "module": "D"}]}}, {"referenceToLCIAMethodDataSet": {"shortDescription": [{"value": "Eutrophication potential terrestrial (EP-terrestrial)", "lang": "en"}, {"value": "Eutrophierungspotenzial Land (EP-terrestrial)", "lang": "de"}], "type": "LCIA method data set", "refObjectId": "b5c614d2-def3-11e6-bf01-fe55135034f3", "uri": "../lciamethods/b5c614d2-def3-11e6-bf01-fe55135034f3.xml"}, "other": {"anies": [{"name": "referenceToUnitGroupDataSet", "value": {"shortDescription": [{"value": "mol N eq", "lang": "en"}], "type": "unit group data set", "refObjectId": "71b4d617-0ec9-4d3f-b65e-e438940c2401", "uri": "../unitgroups/71b4d617-0ec9-4d3f-b65e-e438940c2401.xml"}}, {"value": "1.45689258094429", "module": "A1"}, {"value": "0.0027853572419058", "module": "A2"}, {"value": "0.175115821120273", "module": "A3"}, {"value": "9.0272495371012E-06", "module": "C1"}, {"value": "0.10097221628373", "module": "C2"}, {"value": "0.0286082165518504", "module": "C3"}, {"value": "0.00761056019948661", "module": "C4"}, {"value": "-0.331002326655202", "module": "D"}]}}, {"referenceToLCIAMethodDataSet": {"shortDescription": [{"value": "Formation potential of tropospheric ozone photochemical oxidants (POCP)", "lang": "en"}, {"value": "Bildungspotential für troposphärisches Ozon (POCP)", "lang": "de"}], "type": "LCIA method data set", "refObjectId": "b5c610fe-def3-11e6-bf01-fe55135034f3", "uri": "../lciamethods/b5c610fe-def3-11e6-bf01-fe55135034f3.xml"}, "other": {"anies": [{"name": "referenceToUnitGroupDataSet", "value": {"shortDescription": [{"value": "kg NMVOC eq", "lang": "en"}], "type": "unit group data set", "refObjectId": "d27c25f8-fbc1-44c6-b47b-4adbae4199c6", "uri": "../unitgroups/d27c25f8-fbc1-44c6-b47b-4adbae4199c6.xml"}}, {"value": "0.347874369987495", "module": "A1"}, {"value": "0.000656105423546999", "module": "A2"}, {"value": "0.0401211763661853", "module": "A3"}, {"value": "2.39097060863487E-06", "module": "C1"}, {"value": "0.0169249048635207", "module": "C2"}, {"value": "0.00607553101722705", "module": "C3"}, {"value": "0.0023453886192926", "module": "C4"}, {"value": "-0.0788131103093645", "module": "D"}]}}, {"referenceToLCIAMethodDataSet": {"shortDescription": [{"value": "Abiotic depletion potential for non fossil resources (ADPE)", "lang": "en"}, {"value": "Potenzial für den abiotischen Abbau nicht fossiler Ressourcen (ADPE)", "lang": "de"}], "type": "LCIA method data set", "refObjectId": "b2ad6494-c78d-11e6-9d9d-cec0c932ce01", "uri": "../lciamethods/b2ad6494-c78d-11e6-9d9d-cec0c932ce01.xml"}, "other": {"anies": [{"name": "referenceToUnitGroupDataSet", "value": {"shortDescription": [{"value": "kg Sb eq", "lang": "en"}], "type": "unit group data set", "refObjectId": "54ccd2d9-a32a-4fc2-923d-f2c8c93e89d4", "uri": "../unitgroups/54ccd2d9-a32a-4fc2-923d-f2c8c93e89d4.xml"}}, {"value": "0.00213202162202825", "module": "A1"}, {"value": "4.10648578644774E-08", "module": "A2"}, {"value": "1.39850066462731E-05", "module": "A3"}, {"value": "2.44048859991113E-10", "module": "C1"}, {"value": "2.74909189750739E-07", "module": "C2"}, {"value": "-1.35665383661225E-07", "module": "C3"}, {"value": "3.44736656638948E-08", "module": "C4"}, {"value": "-7.28493524634733E-06", "module": "D"}]}}, {"referenceToLCIAMethodDataSet": {"shortDescription": [{"value": "Abiotic depletion potential for fossil resources (ADPF)", "lang": "en"}, {"value": "Potenzial für den abiotischen Abbau fossiler Brennstoffe (ADPF)", "lang": "de"}], "type": "LCIA method data set", "refObjectId": "b2ad6110-c78d-11e6-9d9d-cec0c932ce01", "uri": "../lciamethods/b2ad6110-c78d-11e6-9d9d-cec0c932ce01.xml"}, "other": {"anies": [{"name": "referenceToUnitGroupDataSet", "value": {"shortDescription": [{"value": "MJ", "lang": "en"}], "type": "unit group data set", "refObjectId": "93a60a57-a3c8-11da-a746-0800200c9a66", "uri": "../unitgroups/93a60a57-a3c8-11da-a746-0800200c9a66.xml"}}, {"value": "1849.41264654354", "module": "A1"}, {"value": "6.23741346063176", "module": "A2"}, {"value": "225.925818412823", "module": "A3"}, {"value": "0.040844514193647", "module": "C1"}, {"value": "41.3119894862957", "module": "C2"}, {"value": "5.36005062818178", "module": "C3"}, {"value": "5.033575826752", "module": "C4"}, {"value": "-449.00279139066", "module": "D"}]}}, {"referenceToLCIAMethodDataSet": {"shortDescription": [{"value": "Water use (WDP)", "lang": "en"}, {"value": "Wassernutzung (WDP)", "lang": "de"}], "type": "LCIA method data set", "refObjectId": "b2ad66ce-c78d-11e6-9d9d-cec0c932ce01", "uri": "../lciamethods/b2ad66ce-c78d-11e6-9d9d-cec0c932ce01.xml"}, "other": {"anies": [{"name": "referenceToUnitGroupDataSet", "value": {"shortDescription": [{"value": "m^(3) world eq deprived", "lang": "en"}], "type": "unit group data set", "refObjectId": "6ae2df01-888e-46c8-b17d-49fa3869b476", "uri": "../unitgroups/6ae2df01-888e-46c8-b17d-49fa3869b476.xml"}}, {"value": "9.31864289788427", "module": "A1"}, {"value": "0.00428529646902343", "module": "A2"}, {"value": "0.694982549067006", "module": "A3"}, {"value": "0.000157854665216823", "module": "C1"}, {"value": "0.0287817528487697", "module": "C2"}, {"value": "2.0731600001868", "module": "C3"}, {"value": "0.0393463474372322", "module": "C4"}, {"value": "-2.0482739635479", "module": "D"}]}}, {"referenceToLCIAMethodDataSet": {"shortDescription": [{"value": "Incidence of disease due to PM emissions (PM)", "lang": "en"}, {"value": "Auftreten von Krankheiten aufgrund von Feinstaubemissionen (PM)", "lang": "de"}], "type": "LCIA method data set", "refObjectId": "b5c602c6-def3-11e6-bf01-fe55135034f3", "uri": "../lciamethods/b5c602c6-def3-11e6-bf01-fe55135034f3.xml"}, "other": {"anies": [{"name": "referenceToUnitGroupDataSet", "value": {"shortDescription": [{"value": "Disease incidence", "lang": "en"}], "type": "unit group data set", "refObjectId": "3883559b-648f-4afc-8ba2-0bd24f3affa3", "uri": "../unitgroups/3883559b-648f-4afc-8ba2-0bd24f3affa3.xml"}}, {"value": "9.22686823637785E-06", "module": "A1"}, {"value": "8.26961570256313E-09", "module": "A2"}, {"value": "4.19823828635639E-07", "module": "A3"}, {"value": "2.90181771034758E-11", "module": "C1"}, {"value": "8.0758871276297E-08", "module": "C2"}, {"value": "3.22419863559379E-08", "module": "C3"}, {"value": "3.18294416641105E-08", "module": "C4"}, {"value": "-1.31400796331112E-06", "module": "D"}]}}, {"referenceToLCIAMethodDataSet": {"shortDescription": [{"value": "Human exposure efficiency relative to U235 (IR)", "lang": "en"}, {"value": "Wirkung durch Exposition des Menschen mit U235 (IR)", "lang": "de"}], "type": "LCIA method data set", "refObjectId": "b5c632be-def3-11e6-bf01-fe55135034f3", "uri": "../lciamethods/b5c632be-def3-11e6-bf01-fe55135034f3.xml"}, "other": {"anies": [{"name": "referenceToUnitGroupDataSet", "value": {"shortDescription": [{"value": "kBq U235 eq", "lang": "en"}], "type": "unit group data set", "refObjectId": "456b05bf-1415-44a9-9993-02452f554c09", "uri": "../unitgroups/456b05bf-1415-44a9-9993-02452f554c09.xml"}}, {"value": "8.87075153132422", "module": "A1"}, {"value": "0.0016493204869054", "module": "A2"}, {"value": "1.51079101268013", "module": "A3"}, {"value": "0.000966201236785339", "module": "C1"}, {"value": "0.0109991300921776", "module": "C2"}, {"value": "0.0279462644117628", "module": "C3"}, {"value": "0.0058566616079903", "module": "C4"}, {"value": "-3.2000175579883", "module": "D"}]}}, {"referenceToLCIAMethodDataSet": {"shortDescription": [{"value": "Comparative toxic unit for ecosystems (ETP-fw)", "lang": "en"}, {"value": "Toxizitätsvergleichseinheit für Ökosysteme (ETP-fw)", "lang": "de"}], "type": "LCIA method data set", "refObjectId": "ee1082d1-b0f7-43ca-a1f0-21e2a4a74511", "uri": "../lciamethods/ee1082d1-b0f7-43ca-a1f0-21e2a4a74511.xml"}, "other": {"anies": [{"name": "referenceToUnitGroupDataSet", "value": {"shortDescription": [{"value": "CTUe", "lang": "en"}], "type": "unit group data set", "refObjectId": "aa959ded-f1eb-4efb-9c5c-2d60be36b3e6", "uri": "../unitgroups/aa959ded-f1eb-4efb-9c5c-2d60be36b3e6.xml"}}, {"value": "2262.97019733333", "module": "A1"}, {"value": "4.62652762721419", "module": "A2"}, {"value": "64.346977115423", "module": "A3"}, {"value": "0.0125450593691226", "module": "C1"}, {"value": "30.6562931006278", "module": "C2"}, {"value": "2.54954403628031", "module": "C3"}, {"value": "3.17095768691364", "module": "C4"}, {"value": "-212.128449688488", "module": "D"}]}}, {"referenceToLCIAMethodDataSet": {"shortDescription": [{"value": "Comparative toxic unit for humans (carcinogenic) (HTP-c)", "lang": "en"}, {"value": "Toxizitätsvergleichseinheit für Menschen (krebserregend) (HTP-c)", "lang": "de"}], "type": "LCIA method data set", "refObjectId": "2299222a-bbd8-474f-9d4f-4dd1f18aea7c", "uri": "../lciamethods/2299222a-bbd8-474f-9d4f-4dd1f18aea7c.xml"}, "other": {"anies": [{"name": "referenceToUnitGroupDataSet", "value": {"shortDescription": [{"value": "CTUh", "lang": "en"}], "type": "unit group data set", "refObjectId": "d4c9523e-2d7e-49fd-8469-998f547d3a70", "uri": "../unitgroups/d4c9523e-2d7e-49fd-8469-998f547d3a70.xml"}}, {"value": "6.53511207950643E-07", "module": "A1"}, {"value": "9.34442817372343E-11", "module": "A2"}, {"value": "9.34803135383842E-09", "module": "A3"}, {"value": "2.09429478099162E-13", "module": "C1"}, {"value": "6.2004038043731E-10", "module": "C2"}, {"value": "1.32106772078573E-10", "module": "C3"}, {"value": "4.00052891286497E-10", "module": "C4"}, {"value": "-2.87174082752285E-08", "module": "D"}]}}, {"referenceToLCIAMethodDataSet": {"shortDescription": [{"value": "Comparative toxic unit for humans (noncarcinogenic) (HTP-nc)", "lang": "en"}, {"value": "Toxizitätsvergleichseinheit für Menschen (nicht krebserregend) (HTP-nc)", "lang": "de"}], "type": "LCIA method data set", "refObjectId": "3af763a5-b7a1-48c9-9cee-1f223481fcef", "uri": "../lciamethods/3af763a5-b7a1-48c9-9cee-1f223481fcef.xml"}, "other": {"anies": [{"name": "referenceToUnitGroupDataSet", "value": {"shortDescription": [{"value": "CTUh", "lang": "en"}], "type": "unit group data set", "refObjectId": "d4c9523e-2d7e-49fd-8469-998f547d3a70", "uri": "../unitgroups/d4c9523e-2d7e-49fd-8469-998f547d3a70.xml"}}, {"value": "2.119102683398E-06", "module": "A1"}, {"value": "4.84140846403672E-09", "module": "A2"}, {"value": "2.19412251729251E-07", "module": "A3"}, {"value": "1.15526883775988E-11", "module": "C1"}, {"value": "3.80016638672308E-08", "module": "C2"}, {"value": "9.0175382465E-09", "module": "C3"}, {"value": "4.4514527408417E-08", "module": "C4"}, {"value": "-2.9596300740751E-07", "module": "D"}]}}, {"referenceToLCIAMethodDataSet": {"shortDescription": [{"value": "Soil quality index (SQP)", "lang": "en"}, {"value": "Bodenqualitätsindex (SQP)", "lang": "de"}], "type": "LCIA method data set", "refObjectId": "b2ad6890-c78d-11e6-9d9d-cec0c932ce01", "uri": "../lciamethods/b2ad6890-c78d-11e6-9d9d-cec0c932ce01.xml"}, "other": {"anies": [{"name": "referenceToUnitGroupDataSet", "value": {"shortDescription": [{"value": "SQP", "lang": "en"}], "type": "unit group data set", "refObjectId": "f130951c-e67f-4f7f-8dd4-665de3974e18", "uri": "../unitgroups/f130951c-e67f-4f7f-8dd4-665de3974e18.xml"}}, {"value": "5204.64403921811", "module": "A1"}, {"value": "2.10780629737533", "module": "A2"}, {"value": "376.048219417024", "module": "A3"}, {"value": "0.00338512642906935", "module": "C1"}, {"value": "14.1992867541184", "module": "C2"}, {"value": "0.228964219784071", "module": "C3"}, {"value": "0.942131324785718", "module": "C4"}, {"value": "-22.4834477062737", "module": "D"}]}}]}, "otherAttributes": {"{http://www.indata.network/EPD/2019}epd-version": "1.2"}, "version": "1.1", "locations": "../ILCDLocations.xml"}