{"processInformation": {"dataSetInformation": {"UUID": "fd6ae0fa-4d2d-4005-9759-909e508751ab", "name": {"baseName": [{"value": "Airium cement-based insulation foam", "lang": "en"}, {"value": "Airium zementbasierter Dämmschaum", "lang": "de"}], "functionalUnitFlowProperties": [{"lang": "en"}]}, "classificationInformation": {"classification": [{"class": [{"value": "Dämmstoffe", "level": 0, "classId": "2"}, {"value": "Ortschaum", "level": 1, "classId": "2.26"}, {"value": "Mineralisch", "level": 2, "classId": "2.26.01"}], "name": "OEKOBAU.DAT"}, {"class": [{"value": "02 Building products", "level": 0}, {"value": "Thermal insulation products", "level": 1}, {"value": "cement-based foams", "level": 2}], "name": "IBUCategories"}]}, "generalComment": [{"value": "Airium™ Spray is an insulating technology that improves the energy efficiency of buildings as part of External Thermal Insulation Composite Systems (ETICS). Airium™ Spray is generated via a continuous chemical foaming reaction by mixing a cement-based dry slurry and a diluted solution of hydrogen peroxide with a dedicated equipment.\n\nAirium™ Spray is the first mineral foam to offer a top-tier insulating performance and which can be applied on vertical surfaces. Airium™ Spray, within a full system approach developed through a partnership between Holcim and HASIT Group, aims to fulfil all core requirements of ETICS in new-build and in renovation projects: \nit is an efficient insulator in cold and hot weather. It also has a superior thermal phase shift (14 hours) than wool and polystyrene alternatives;\nit is ranked A1 and is fully fire resistant;\nit contains no harmful fibres, emits no volatile organic compounds (VOCs) and is a breathable material that limits the risk of mould;\nit provides a continuous insulation layer with no thermal bridges;\nit insulates efficiently over time as it is dimensionally stable and does not settle or sag;\nit accelerates the time required to place insulation on site by a factor of 2 while diminishing waste and storage space required on site;\nit is resistant to insects or rodents;\nit is highly insulating over time and recyclable, in cement, in concrete or in Airium™ with no separation phase.", "lang": "en"}], "other": {"anies": [{"scenario": [{"description": [{"value": "100% Recycling", "lang": "en"}, {"value": "100% Recycling", "lang": "de"}], "name": "S1", "default": true}, {"description": [{"value": "100% Landfilling", "lang": "en"}, {"value": "100% Deponie", "lang": "de"}], "name": "S2"}]}]}}, "quantitativeReference": {"referenceToReferenceFlow": [0]}, "time": {"referenceYear": 2022, "dataSetValidUntil": 2027, "other": {"anies": [{"name": "publicationDateOfEPD", "value": 1663718400000}]}}, "geography": {"locationOfOperationSupplyOrProduction": {"location": "RER"}}, "technology": {"technologyDescriptionAndIncludedProcesses": [{"value": "The raw materials are stored at the manufacturing plant in silos or IBCs. From the silos, the raw materials are dosed and intensely mixed according to the formulation. The mixture is then packaged and shipped in packages or in a silo. The manufacturing process of the premix is illustrated using the following graphic. \nDeclared unit: \nThe declared unit is 1 m3 at a density of 100 kg/m3 (after drying curing).", "lang": "en"}, {"value": "Die Rohstoffe werden in der Produktionsstätte in Silos oder IBCs gelagert. Aus den Silos werden die Rohstoffe entsprechend der Rezeptur dosiert und intensiv gemischt. Die Mischung wird dann verpackt und in Paketen oder in einem Silo verschickt. \n\n\nDer Herstellungsprozess der Vormischung wird anhand der folgenden Grafik veranschaulicht. \n", "lang": "de"}], "technologicalApplicability": [{"value": "Airium™ Spray is a cement-based insulation foam produced on site and applied by hand. It can be used for retrofitting and new construction. The insulation after hardening can be covered with claddings or plastered with specialized mortar and components used for ETICS. \n\nFor use in old and new building insulation: \n\nAs system component in the thermal insulation composite system (ETICS)\nInterior and exterior insulation of outside walls\nDouble-wall masonry\nWall cavity insulation\nVentilated curtain facades", "lang": "en"}, {"value": "Airium™ Spray ist ein zementbasierter Dämmschaum, der vor Ort hergestellt und von Hand aufgetragen wird. Er kann für die Nachrüstung und für Neubauten verwendet werden. Die Dämmung kann nach dem Aushärten mit Verkleidungen überzogen oder mit Spezialmörtel und Komponenten für WDVS verputzt werden.\n\nFür den Einsatz in der Alt- und Neubaudämmung:\n\nAls Systemkomponente im Wärmedämmverbundsystem (WDVS)\nInnen- und Außendämmung von Außenwänden\nZweischaliges Mauerwerk\nWandhohlraumdämmung\nHinterlüftete Vorhangfassaden", "lang": "de"}]}}, "modellingAndValidation": {"LCIMethodAndAllocation": {"typeOfDataSet": "EPD", "referenceToLCAMethodDetails": [{"shortDescription": [{"value": "cement-based foams.pdf", "lang": "en"}], "type": "source data set", "refObjectId": "cb825841-6521-499e-b6a2-fe1d48eee3f9"}], "other": {"anies": [{"name": "subType", "value": "specific dataset"}]}}, "dataSourcesTreatmentAndRepresentativeness": {"referenceToDataSource": [{"shortDescription": [{"value": "ecoinvent database (all versions)", "lang": "en"}], "type": "source data set", "refObjectId": "b497a91f-e14b-4b69-8f28-f50eb1576766"}, {"shortDescription": [{"value": "ecoinvent 3.8 database", "lang": "en"}], "type": "source data set", "refObjectId": "0f4c65c0-6210-450f-b886-82bf8dd5ace9"}], "useAdviceForDataSet": [{"value": "Scope: \nAirium™ Spray is a cement-based insulation foam produced on site by mixing two components: a dry slurry made with premix and water and a diluted solution of hydrogen peroxide. The life cycle assessment is based on components produced in different plants and on-site production data. The premix is produced by HASIT (plant located in Kissing, Germany) with cement produced by Holcim Germany (plant located in Dotternhausen, Germany), and additives produced by other suppliers. The diluted solution of hydrogen peroxide is produced by Solvay (the foreground data are primary production data from Solvay industrial sites in Europe). \nSystem boundary: \nA life cycle assessment type „cradle to gate with options, with modules C1 – C4, and module D (A1-A3, C1-C3, D and additional modules” is calculated. \n\n\nModules A1-A3 contain the production of the dry slurry and the additive based on (H2O2) as well as the packaging (15% of the dry slurry packed in paper bags, 85% of the dry slurry filled into a dual silo together with the additive); it also includes the production of the silo (and the associated machinery for mixing/installation (allocated based on the estimated total turn-over over their service life). \n\n\nModule A4 includes the transport of the two components and the silo/machinery to the construction site. \n\n\nModule A5 covers the mixing of the two components, its installation, the landfilling of the installation (waste) as well as the thermal treatment of the paper bags used for packaging in a municipal waste incineration part. Due to the very limited amount, no exported energy is declared in A5 nor considered in module D. \n\n\nModule B1 includes the carbonation of the cementitious foam. \n\n\nModule C1: Mechanical deconstruction is assumed, implying the consumption of diesel in a building machine and some dust emissions. \n\n\nIn Module C2, it is assumed that the de-installed product is transported to an inert material landfill (scenario 1) or to a sorting platform over 50 km for recycling (scenario 2). \n\n\nModule C3_2: For the 100% recycling scenario (scenario 2), it is assumed that the deconstructed wall including the insulation material are sorted in a sorting plant; during this process, the insulation material will be converted into a homogeneous powder that reaches “end-of-waste”. It can be further used as a filler in cement or mortar production. \n\n\nModule C4_1: For the 100% landfilling scenario (scenario 1), it is assumed that the deinstalled product is disposed of in a landfill for inert materials. \n\n\nModule D_2: For the recycling scenario, a substitution of milled limestone used in the production of cement or mortar is assumed.", "lang": "en"}], "other": {"anies": [{"name": "referenceToOriginalEPD", "value": {"shortDescription": {"value": "Airium cement-based insulation foam.pdf", "defaultValue": "Airium cement-based insulation foam.pdf", "lstrings": [{"lang": "en", "value": "Airium cement-based insulation foam.pdf"}]}, "type": "source data set", "uuid": {"uuid": "609e78c3-7001-4962-a4e1-a79413f98fab"}, "refObjectId": "609e78c3-7001-4962-a4e1-a79413f98fab", "resourceURLs": ["https://oekobaudat.de/OEKOBAU.DAT/resource/sources/609e78c3-7001-4962-a4e1-a79413f98fab/Airium_cement-based_insulation_foam_15663.pdf?version=00.01.000"]}}]}}, "validation": {"review": [{"referenceToNameOfReviewerAndInstitution": [{"shortDescription": [{"value": "Institut Bauen und Umwelt e. V.", "lang": "en"}], "type": "contact data set", "refObjectId": "d111dbec-b024-4be5-86c5-752d6eb2cf95", "uri": "../contacts/d111dbec-b024-4be5-86c5-752d6eb2cf95.xml"}], "type": "Accredited third party review"}]}, "complianceDeclarations": {"compliance": [{"referenceToComplianceSystem": {"shortDescription": [{"value": "DIN EN 15804+A2", "lang": "en"}], "type": "source data set", "refObjectId": "c0016b33-8cf7-415c-ac6e-deba0d21440d", "uri": "../sources/c0016b33-8cf7-415c-ac6e-deba0d21440d.xml"}}, {"referenceToComplianceSystem": {"shortDescription": [{"value": "ISO 14025", "lang": "en"}], "type": "source data set", "refObjectId": "4f2eb655-6e44-4874-a95a-e28f5442cd4d", "uri": "../sources/4f2eb655-6e44-4874-a95a-e28f5442cd4d.xml"}}]}}, "administrativeInformation": {"commissionerAndGoal": {"referenceToCommissioner": [{"shortDescription": [{"value": "Holcim (Deutschland) GmbH", "lang": "en"}], "type": "contact data set", "refObjectId": "8ac54d9c-9919-4aba-8f9c-837b3225cd67", "uri": "../contacts/8ac54d9c-9919-4aba-8f9c-837b3225cd67.xml"}]}, "dataGenerator": {"referenceToPersonOrEntityGeneratingTheDataSet": [{"shortDescription": [{"value": "Dr. Frank Werner - Umwelt & Entwicklung", "lang": "en"}], "type": "contact data set", "refObjectId": "62792478-795c-4ae2-ac9a-1012d9515424", "uri": "../contacts/62792478-795c-4ae2-ac9a-1012d9515424.xml"}]}, "dataEntryBy": {"timeStamp": 1663766308387, "referenceToDataSetFormat": [{"shortDescription": [{"value": "ILCD Format", "lang": "en"}], "type": "source data set", "refObjectId": "a97a0155-0234-4b87-b4ce-a45da52f2a40", "uri": "../sources/a97a0155-0234-4b87-b4ce-a45da52f2a40.xml"}, {"shortDescription": [{"value": "EPD-Datenformaterweiterungen v1.2", "lang": "de"}, {"value": "EPD Data Format Extensions v1.2", "lang": "en"}], "type": "source data set", "refObjectId": "a29449fd-aa2f-4de8-b5d7-4b06b43c6fde", "uri": "../sources/a29449fd-aa2f-4de8-b5d7-4b06b43c6fde.xml"}]}, "publicationAndOwnership": {"dataSetVersion": "00.01.000", "referenceToRegistrationAuthority": {"shortDescription": [{"value": "Institut Bauen und Umwelt e. V.", "lang": "en"}], "type": "contact data set", "refObjectId": "d111dbec-b024-4be5-86c5-752d6eb2cf95", "uri": "../contacts/d111dbec-b024-4be5-86c5-752d6eb2cf95.xml"}, "registrationNumber": "EPD-HOC-20220204-IBD1-EN", "referenceToOwnershipOfDataSet": {"shortDescription": [{"value": "Holcim (Deutschland) GmbH", "lang": "en"}], "type": "contact data set", "refObjectId": "8ac54d9c-9919-4aba-8f9c-837b3225cd67", "uri": "../contacts/8ac54d9c-9919-4aba-8f9c-837b3225cd67.xml"}, "copyright": true, "licenseType": "Free of charge for all users and uses", "accessRestrictions": [{"value": "None", "lang": "en"}], "other": {"anies": [{"name": "referenceToPublisher", "value": {"shortDescription": [{"value": "Institut Bauen und Umwelt e. V.", "lang": "en"}], "type": "contact data set", "refObjectId": "d111dbec-b024-4be5-86c5-752d6eb2cf95", "uri": "../contacts/d111dbec-b024-4be5-86c5-752d6eb2cf95.xml"}}]}}}, "exchanges": {"exchange": [{"dataSetInternalID": 0, "referenceToFlowDataSet": {"shortDescription": [{"value": "Airium™ cement-based insulation foam 100 kg/m³ ()", "lang": "en"}], "type": "flow data set", "refObjectId": "9317c41a-0d3d-3824-056d-444eadcb5d84", "uri": "../flows/9317c41a-0d3d-3824-056d-444eadcb5d84.xml"}, "meanAmount": 1.0, "referencesToDataSource": {}, "referenceFlow": true, "resolvedFlowVersion": "00.01.000", "resultingflowAmount": 1.0, "flowProperties": [{"name": [{"lang": "en", "value": "Volume"}, {"lang": "de", "value": "Volumen"}], "uuid": "93a60a56-a3c8-22da-a746-0800200c9a66", "referenceFlowProperty": true, "meanValue": 1.0, "referenceUnit": "m3", "unitGroupUUID": "cd950537-0a98-4044-9ba7-9f9a68d0a504"}], "materialProperties": [{"name": "gross density", "value": "100.0", "unit": "kg/m^3", "unitDescription": "kilograms per cubic metre"}], "typeOfFlow": "Product flow", "classification": {"classHierarchy": "Dämmstoffe / Ortschaum / Mineralisch", "name": "OEKOBAU.DAT"}}, {"dataSetInternalID": 1, "referenceToFlowDataSet": {"shortDescription": [{"value": "Renewable primary energy as energy carrier (PERE)", "lang": "en"}, {"value": "Erneuerbare Primärenergie als Energieträger (PERE)", "lang": "de"}], "type": "flow data set", "refObjectId": "20f32be5-0398-4288-9b6d-accddd195317", "uri": "../flows/20f32be5-0398-4288-9b6d-accddd195317.xml"}, "exchange direction": "INPUT", "other": {"anies": [{"name": "referenceToUnitGroupDataSet", "value": {"shortDescription": [{"value": "MJ", "lang": "en"}], "type": "unit group data set", "refObjectId": "93a60a57-a3c8-11da-a746-0800200c9a66", "uri": "../unitgroups/93a60a57-a3c8-11da-a746-0800200c9a66.xml"}}, {"value": "17.0296987724557", "module": "A1-A3"}, {"value": "1.05577778351238", "module": "A4"}, {"value": "0.00174050850081625", "module": "A5"}, {"value": "0", "module": "B1"}, {"value": "0.0300651407632493", "module": "C1"}, {"value": "0.208092191878915", "module": "C2"}, {"value": "1.6499475512539", "module": "C3"}, {"value": "0.325961282247927", "module": "C4"}, {"value": "0", "module": "D", "scenario": "S1"}, {"value": "-7.01102420544441", "module": "D", "scenario": "S2"}]}, "resolvedFlowVersion": "38.00.000", "flowProperties": [], "typeOfFlow": "Other flow", "classification": {"classHierarchy": "Quantities", "name": "GaBiCategories"}}, {"dataSetInternalID": 2, "referenceToFlowDataSet": {"shortDescription": [{"value": "Renewable primary energy resources as material utilization (PERM)", "lang": "en"}, {"value": "Erneuerbare Primärenergie zur stofflichen Nutzung (PERM)", "lang": "de"}], "type": "flow data set", "refObjectId": "fb3ec0de-548d-4508-aea5-00b73bf6f702", "uri": "../flows/fb3ec0de-548d-4508-aea5-00b73bf6f702.xml"}, "exchange direction": "INPUT", "other": {"anies": [{"name": "referenceToUnitGroupDataSet", "value": {"shortDescription": [{"value": "MJ", "lang": "en"}], "type": "unit group data set", "refObjectId": "93a60a57-a3c8-11da-a746-0800200c9a66", "uri": "../unitgroups/93a60a57-a3c8-11da-a746-0800200c9a66.xml"}}, {"value": "0", "module": "A1-A3"}, {"value": "0", "module": "A4"}, {"value": "0", "module": "A5"}, {"value": "0", "module": "B1"}, {"value": "0", "module": "C1"}, {"value": "0", "module": "C2"}, {"value": "0", "module": "C3"}, {"value": "0", "module": "C4"}, {"value": "0", "module": "D", "scenario": "S1"}, {"value": "0", "module": "D", "scenario": "S2"}]}, "resolvedFlowVersion": "38.00.000", "flowProperties": [], "typeOfFlow": "Other flow", "classification": {"classHierarchy": "Quantities", "name": "GaBiCategories"}}, {"dataSetInternalID": 3, "referenceToFlowDataSet": {"shortDescription": [{"value": "Total use of renewable primary energy resources (PERT)", "lang": "en"}, {"value": "Total erneuerbare Primärenergie (PERT)", "lang": "de"}], "type": "flow data set", "refObjectId": "53f97275-fa8a-4cdd-9024-65936002acd0", "uri": "../flows/53f97275-fa8a-4cdd-9024-65936002acd0.xml"}, "exchange direction": "INPUT", "other": {"anies": [{"name": "referenceToUnitGroupDataSet", "value": {"shortDescription": [{"value": "MJ", "lang": "en"}], "type": "unit group data set", "refObjectId": "93a60a57-a3c8-11da-a746-0800200c9a66", "uri": "../unitgroups/93a60a57-a3c8-11da-a746-0800200c9a66.xml"}}, {"value": "17.0296987724557", "module": "A1-A3"}, {"value": "1.05577778351238", "module": "A4"}, {"value": "0.00174050850081625", "module": "A5"}, {"value": "0", "module": "B1"}, {"value": "0.0300651407632493", "module": "C1"}, {"value": "0.208092191878915", "module": "C2"}, {"value": "1.6499475512539", "module": "C3"}, {"value": "0.325961282247927", "module": "C4"}, {"value": "0", "module": "D", "scenario": "S1"}, {"value": "-7.01102420544441", "module": "D", "scenario": "S2"}]}, "resolvedFlowVersion": "38.00.000", "flowProperties": [], "typeOfFlow": "Other flow", "classification": {"classHierarchy": "Quantities / Environmental quantities / EPD EN 15804 / LCI indicators", "name": "GaBiCategories"}}, {"dataSetInternalID": 4, "referenceToFlowDataSet": {"shortDescription": [{"value": "Non renewable primary energy as energy carrier (PENRE)", "lang": "en"}, {"value": "Nicht-erneuerbare Primärenergie als Energieträger (PENRE)", "lang": "de"}], "type": "flow data set", "refObjectId": "ac857178-2b45-46ec-892a-a9a4332f0372", "uri": "../flows/ac857178-2b45-46ec-892a-a9a4332f0372.xml"}, "exchange direction": "INPUT", "other": {"anies": [{"name": "referenceToUnitGroupDataSet", "value": {"shortDescription": [{"value": "MJ", "lang": "en"}], "type": "unit group data set", "refObjectId": "93a60a57-a3c8-11da-a746-0800200c9a66", "uri": "../unitgroups/93a60a57-a3c8-11da-a746-0800200c9a66.xml"}}, {"value": "287.629935044313", "module": "A1-A3"}, {"value": "75.1232588755338", "module": "A4"}, {"value": "0.0357666628384521", "module": "A5"}, {"value": "0", "module": "B1"}, {"value": "5.42954648172739", "module": "C1"}, {"value": "14.8066798190148", "module": "C2"}, {"value": "13.9153890473471", "module": "C3"}, {"value": "16.4738600958071", "module": "C4"}, {"value": "0", "module": "D", "scenario": "S1"}, {"value": "-44.271831246711", "module": "D", "scenario": "S2"}]}, "resolvedFlowVersion": "38.00.000", "flowProperties": [], "typeOfFlow": "Other flow", "classification": {"classHierarchy": "Quantities", "name": "GaBiCategories"}}, {"dataSetInternalID": 5, "referenceToFlowDataSet": {"shortDescription": [{"value": "Non renewable primary energy as material utilization (PENRM)", "lang": "en"}, {"value": "Nicht-erneuerbare Primärenergie zur stofflichen Nutzung (PENRM)", "lang": "de"}], "type": "flow data set", "refObjectId": "1421caa0-679d-4bf4-b282-0eb850ccae27", "uri": "../flows/1421caa0-679d-4bf4-b282-0eb850ccae27.xml"}, "exchange direction": "INPUT", "other": {"anies": [{"name": "referenceToUnitGroupDataSet", "value": {"shortDescription": [{"value": "MJ", "lang": "en"}], "type": "unit group data set", "refObjectId": "93a60a57-a3c8-11da-a746-0800200c9a66", "uri": "../unitgroups/93a60a57-a3c8-11da-a746-0800200c9a66.xml"}}, {"value": "0", "module": "A1-A3"}, {"value": "0", "module": "A4"}, {"value": "0", "module": "A5"}, {"value": "0", "module": "B1"}, {"value": "0", "module": "C1"}, {"value": "0", "module": "C2"}, {"value": "0", "module": "C3"}, {"value": "0", "module": "C4"}, {"value": "0", "module": "D", "scenario": "S1"}, {"value": "0", "module": "D", "scenario": "S2"}]}, "resolvedFlowVersion": "38.00.000", "flowProperties": [], "typeOfFlow": "Other flow", "classification": {"classHierarchy": "Quantities", "name": "GaBiCategories"}}, {"dataSetInternalID": 6, "referenceToFlowDataSet": {"shortDescription": [{"value": "Total use of non renewable primary energy resources (PENRT)", "lang": "en"}, {"value": "Total nicht erneuerbare Primärenergie (PENRT)", "lang": "de"}], "type": "flow data set", "refObjectId": "06159210-646b-4c8d-8583-da9b3b95a6c1", "uri": "../flows/06159210-646b-4c8d-8583-da9b3b95a6c1.xml"}, "exchange direction": "INPUT", "other": {"anies": [{"name": "referenceToUnitGroupDataSet", "value": {"shortDescription": [{"value": "MJ", "lang": "en"}], "type": "unit group data set", "refObjectId": "93a60a57-a3c8-11da-a746-0800200c9a66", "uri": "../unitgroups/93a60a57-a3c8-11da-a746-0800200c9a66.xml"}}, {"value": "287.629935044313", "module": "A1-A3"}, {"value": "75.1232588755338", "module": "A4"}, {"value": "0.0357666628384521", "module": "A5"}, {"value": "0", "module": "B1"}, {"value": "5.42954648172739", "module": "C1"}, {"value": "14.8066798190148", "module": "C2"}, {"value": "13.9153890473471", "module": "C3"}, {"value": "16.4738600958071", "module": "C4"}, {"value": "0", "module": "D", "scenario": "S1"}, {"value": "-44.271831246711", "module": "D", "scenario": "S2"}]}, "resolvedFlowVersion": "38.00.000", "flowProperties": [], "typeOfFlow": "Other flow", "classification": {"classHierarchy": "Quantities / Environmental quantities / EPD EN 15804 / LCI indicators", "name": "GaBiCategories"}}, {"dataSetInternalID": 7, "referenceToFlowDataSet": {"shortDescription": [{"value": "Use of secondary material (SM)", "lang": "en"}, {"value": "Einsatz von Sekundärstoffen (SM)", "lang": "de"}], "type": "flow data set", "refObjectId": "c6a1f35f-2d09-4f54-8dfb-97e502e1ce92", "uri": "../flows/c6a1f35f-2d09-4f54-8dfb-97e502e1ce92.xml"}, "exchange direction": "INPUT", "other": {"anies": [{"name": "referenceToUnitGroupDataSet", "value": {"shortDescription": [{"value": "kg", "lang": "en"}], "type": "unit group data set", "refObjectId": "ad38d542-3fe9-439d-9b95-2f5f7752acaf", "uri": "../unitgroups/ad38d542-3fe9-439d-9b95-2f5f7752acaf.xml"}}, {"value": "0", "module": "A1-A3"}, {"value": "0", "module": "A4"}, {"value": "0", "module": "A5"}, {"value": "0", "module": "B1"}, {"value": "0", "module": "C1"}, {"value": "0", "module": "C2"}, {"value": "0", "module": "C3"}, {"value": "0", "module": "C4"}, {"value": "0", "module": "D", "scenario": "S1"}, {"value": "119.9", "module": "D", "scenario": "S2"}]}, "resolvedFlowVersion": "38.00.000", "flowProperties": [], "typeOfFlow": "Other flow", "classification": {"classHierarchy": "Quantities / Environmental quantities / EPD EN 15804 / LCI indicators", "name": "GaBiCategories"}}, {"dataSetInternalID": 8, "referenceToFlowDataSet": {"shortDescription": [{"value": "Use of renewable secondary fuels (RSF)", "lang": "en"}, {"value": "Erneuerbare Sekundärbrennstoffe (RSF)", "lang": "de"}], "type": "flow data set", "refObjectId": "64333088-a55f-4aa2-9a31-c10b07816787", "uri": "../flows/64333088-a55f-4aa2-9a31-c10b07816787.xml"}, "exchange direction": "INPUT", "other": {"anies": [{"name": "referenceToUnitGroupDataSet", "value": {"shortDescription": [{"value": "MJ", "lang": "en"}], "type": "unit group data set", "refObjectId": "93a60a57-a3c8-11da-a746-0800200c9a66", "uri": "../unitgroups/93a60a57-a3c8-11da-a746-0800200c9a66.xml"}}, {"value": "0", "module": "A1-A3"}, {"value": "0", "module": "A4"}, {"value": "0", "module": "A5"}, {"value": "0", "module": "B1"}, {"value": "0", "module": "C1"}, {"value": "0", "module": "C2"}, {"value": "0", "module": "C3"}, {"value": "0", "module": "C4"}, {"value": "0", "module": "D", "scenario": "S1"}, {"value": "0", "module": "D", "scenario": "S2"}]}, "resolvedFlowVersion": "38.00.000", "flowProperties": [], "typeOfFlow": "Other flow", "classification": {"classHierarchy": "Quantities / Environmental quantities / EPD EN 15804 / LCI indicators", "name": "GaBiCategories"}}, {"dataSetInternalID": 9, "referenceToFlowDataSet": {"shortDescription": [{"value": "Use of non renewable secondary fuels (NRSF)", "lang": "en"}, {"value": "Nicht erneuerbare Sekundärbrennstoffe (NRSF)", "lang": "de"}], "type": "flow data set", "refObjectId": "89def144-d39a-4287-b86f-efde453ddcb2", "uri": "../flows/89def144-d39a-4287-b86f-efde453ddcb2.xml"}, "exchange direction": "INPUT", "other": {"anies": [{"name": "referenceToUnitGroupDataSet", "value": {"shortDescription": [{"value": "MJ", "lang": "en"}], "type": "unit group data set", "refObjectId": "93a60a57-a3c8-11da-a746-0800200c9a66", "uri": "../unitgroups/93a60a57-a3c8-11da-a746-0800200c9a66.xml"}}, {"value": "0", "module": "A1-A3"}, {"value": "0", "module": "A4"}, {"value": "0", "module": "A5"}, {"value": "0", "module": "B1"}, {"value": "0", "module": "C1"}, {"value": "0", "module": "C2"}, {"value": "0", "module": "C3"}, {"value": "0", "module": "C4"}, {"value": "0", "module": "D", "scenario": "S1"}, {"value": "0", "module": "D", "scenario": "S2"}]}, "resolvedFlowVersion": "38.00.000", "flowProperties": [], "typeOfFlow": "Other flow", "classification": {"classHierarchy": "Quantities / Environmental quantities / EPD EN 15804 / LCI indicators", "name": "GaBiCategories"}}, {"dataSetInternalID": 10, "referenceToFlowDataSet": {"shortDescription": [{"value": "Use of net fresh water (FW)", "lang": "en"}, {"value": "Einsatz von Süßwasserressourcen (FW)", "lang": "de"}], "type": "flow data set", "refObjectId": "3cf952c8-f3a4-461d-8c96-96456ca62246", "uri": "../flows/3cf952c8-f3a4-461d-8c96-96456ca62246.xml"}, "exchange direction": "INPUT", "other": {"anies": [{"name": "referenceToUnitGroupDataSet", "value": {"shortDescription": [{"value": "m^3", "lang": "en"}], "type": "unit group data set", "refObjectId": "cd950537-0a98-4044-9ba7-9f9a68d0a504", "uri": "../unitgroups/cd950537-0a98-4044-9ba7-9f9a68d0a504.xml"}}, {"value": "0.114295062383032", "module": "A1-A3"}, {"value": "0.00668881812682384", "module": "A4"}, {"value": "5.52020591292094E-06", "module": "A5"}, {"value": "0", "module": "B1"}, {"value": "0.000309172197351398", "module": "C1"}, {"value": "0.00131835585747943", "module": "C2"}, {"value": "0.000926569646122411", "module": "C3"}, {"value": "0.00064482682873486", "module": "C4"}, {"value": "0", "module": "D", "scenario": "S1"}, {"value": "-0.00552601093715962", "module": "D", "scenario": "S2"}]}, "resolvedFlowVersion": "38.00.000", "flowProperties": [], "typeOfFlow": "Other flow", "classification": {"classHierarchy": "Quantities / Environmental quantities / EPD EN 15804 / LCI indicators", "name": "GaBiCategories"}}, {"dataSetInternalID": 11, "referenceToFlowDataSet": {"shortDescription": [{"value": "Hazardous waste disposed (HWD)", "lang": "en"}, {"value": "Gefährlicher Abfall zur Deponie (HWD)", "lang": "de"}], "type": "flow data set", "refObjectId": "430f9e0f-59b2-46a0-8e0d-55e0e84948fc", "uri": "../flows/430f9e0f-59b2-46a0-8e0d-55e0e84948fc.xml"}, "exchange direction": "OUTPUT", "other": {"anies": [{"name": "referenceToUnitGroupDataSet", "value": {"shortDescription": [{"value": "kg", "lang": "en"}], "type": "unit group data set", "refObjectId": "ad38d542-3fe9-439d-9b95-2f5f7752acaf", "uri": "../unitgroups/ad38d542-3fe9-439d-9b95-2f5f7752acaf.xml"}}, {"value": "0.000294147462419812", "module": "A1-A3"}, {"value": "0.000196033693438781", "module": "A4"}, {"value": "1.21316615209177E-07", "module": "A5"}, {"value": "0", "module": "B1"}, {"value": "1.48714190437872E-05", "module": "C1"}, {"value": "3.86379421757523E-05", "module": "C2"}, {"value": "3.41392575998218E-05", "module": "C3"}, {"value": "1.82518459493773E-05", "module": "C4"}, {"value": "0", "module": "D", "scenario": "S1"}, {"value": "-2.85899092368012E-05", "module": "D", "scenario": "S2"}]}, "resolvedFlowVersion": "38.00.000", "flowProperties": [], "typeOfFlow": "Other flow", "classification": {"classHierarchy": "Quantities / Environmental quantities / EPD EN 15804 / LCI indicators", "name": "GaBiCategories"}}, {"dataSetInternalID": 12, "referenceToFlowDataSet": {"shortDescription": [{"value": "Non hazardous waste disposed (NHWD)", "lang": "en"}, {"value": "Entsorgter nicht gefährlicher Abfall (NHWD)", "lang": "de"}], "type": "flow data set", "refObjectId": "b29ef66b-e286-4afa-949f-62f1a7b4d7fa", "uri": "../flows/b29ef66b-e286-4afa-949f-62f1a7b4d7fa.xml"}, "exchange direction": "OUTPUT", "other": {"anies": [{"name": "referenceToUnitGroupDataSet", "value": {"shortDescription": [{"value": "kg", "lang": "en"}], "type": "unit group data set", "refObjectId": "ad38d542-3fe9-439d-9b95-2f5f7752acaf", "uri": "../unitgroups/ad38d542-3fe9-439d-9b95-2f5f7752acaf.xml"}}, {"value": "6.62746764570045", "module": "A1-A3"}, {"value": "3.95343430302026", "module": "A4"}, {"value": "0.00309832553509788", "module": "A5"}, {"value": "0", "module": "B1"}, {"value": "0.00903082930226473", "module": "C1"}, {"value": "0.779215875170129", "module": "C2"}, {"value": "0.377670846287888", "module": "C3"}, {"value": "119.834230847102", "module": "C4"}, {"value": "0", "module": "D", "scenario": "S1"}, {"value": "-0.206237057520854", "module": "D", "scenario": "S2"}]}, "resolvedFlowVersion": "38.00.000", "flowProperties": [], "typeOfFlow": "Other flow", "classification": {"classHierarchy": "Quantities / Environmental quantities / EPD EN 15804 / LCI indicators", "name": "GaBiCategories"}}, {"dataSetInternalID": 13, "referenceToFlowDataSet": {"shortDescription": [{"value": "Radioactive waste disposed (RWD)", "lang": "en"}, {"value": "Entsorgter radioaktiver Abfall (RWD)", "lang": "de"}], "type": "flow data set", "refObjectId": "3449546e-52ad-4b39-b809-9fb77cea8ff6", "uri": "../flows/3449546e-52ad-4b39-b809-9fb77cea8ff6.xml"}, "exchange direction": "OUTPUT", "other": {"anies": [{"name": "referenceToUnitGroupDataSet", "value": {"shortDescription": [{"value": "kg", "lang": "en"}], "type": "unit group data set", "refObjectId": "ad38d542-3fe9-439d-9b95-2f5f7752acaf", "uri": "../unitgroups/ad38d542-3fe9-439d-9b95-2f5f7752acaf.xml"}}, {"value": "0.00164394804232561", "module": "A1-A3"}, {"value": "0.00108656875032245", "module": "A4"}, {"value": "3.29622244253183E-07", "module": "A5"}, {"value": "0", "module": "B1"}, {"value": "8.07277986452571E-05", "module": "C1"}, {"value": "0.000214161044504572", "module": "C2"}, {"value": "0.00021888564669826", "module": "C3"}, {"value": "0.000238308904510206", "module": "C4"}, {"value": "0", "module": "D", "scenario": "S1"}, {"value": "-0.000518513451436837", "module": "D", "scenario": "S2"}]}, "resolvedFlowVersion": "38.00.000", "flowProperties": [], "typeOfFlow": "Other flow", "classification": {"classHierarchy": "Quantities / Environmental quantities / EPD EN 15804 / LCI indicators", "name": "GaBiCategories"}}, {"dataSetInternalID": 14, "referenceToFlowDataSet": {"shortDescription": [{"value": "Components for re-use (CRU)", "lang": "en"}, {"value": "Komponenten für die Wiederverwendung (CRU)", "lang": "de"}], "type": "flow data set", "refObjectId": "a2b32f97-3fc7-4af2-b209-525bc6426f33", "uri": "../flows/a2b32f97-3fc7-4af2-b209-525bc6426f33.xml"}, "exchange direction": "OUTPUT", "other": {"anies": [{"name": "referenceToUnitGroupDataSet", "value": {"shortDescription": [{"value": "kg", "lang": "en"}], "type": "unit group data set", "refObjectId": "ad38d542-3fe9-439d-9b95-2f5f7752acaf", "uri": "../unitgroups/ad38d542-3fe9-439d-9b95-2f5f7752acaf.xml"}}, {"value": "0", "module": "A1-A3"}, {"value": "0", "module": "A4"}, {"value": "0", "module": "A5"}, {"value": "0", "module": "B1"}, {"value": "0", "module": "C1"}, {"value": "0", "module": "C2"}, {"value": "0", "module": "C3"}, {"value": "0", "module": "C4"}, {"value": "0", "module": "D", "scenario": "S1"}, {"value": "0", "module": "D", "scenario": "S2"}]}, "resolvedFlowVersion": "38.00.000", "flowProperties": [], "typeOfFlow": "Other flow", "classification": {"classHierarchy": "Quantities / Environmental quantities / EPD EN 15804 / LCI indicators", "name": "GaBiCategories"}}, {"dataSetInternalID": 15, "referenceToFlowDataSet": {"shortDescription": [{"value": "Materials for recycling (MFR)", "lang": "en"}, {"value": "Stoffe zum Recycling (MFR)", "lang": "de"}], "type": "flow data set", "refObjectId": "d7fe48a5-4103-49c8-9aae-b0b5dfdbd6ae", "uri": "../flows/d7fe48a5-4103-49c8-9aae-b0b5dfdbd6ae.xml"}, "exchange direction": "OUTPUT", "other": {"anies": [{"name": "referenceToUnitGroupDataSet", "value": {"shortDescription": [{"value": "kg", "lang": "en"}], "type": "unit group data set", "refObjectId": "ad38d542-3fe9-439d-9b95-2f5f7752acaf", "uri": "../unitgroups/ad38d542-3fe9-439d-9b95-2f5f7752acaf.xml"}}, {"value": "0", "module": "A1-A3"}, {"value": "0", "module": "A4"}, {"value": "0", "module": "A5"}, {"value": "0", "module": "B1"}, {"value": "0", "module": "C1"}, {"value": "0", "module": "C2"}, {"value": "119.9", "module": "C3"}, {"value": "0", "module": "C4"}, {"value": "0", "module": "D", "scenario": "S1"}, {"value": "0", "module": "D", "scenario": "S2"}]}, "resolvedFlowVersion": "38.00.000", "flowProperties": [], "typeOfFlow": "Other flow", "classification": {"classHierarchy": "Quantities / Environmental quantities / EPD EN 15804 / LCI indicators", "name": "GaBiCategories"}}, {"dataSetInternalID": 16, "referenceToFlowDataSet": {"shortDescription": [{"value": "Materials for energy recovery (MER)", "lang": "en"}, {"value": "Stoffe für die Energierückgewinnung (MER)", "lang": "de"}], "type": "flow data set", "refObjectId": "59a9181c-3aaf-46ee-8b13-2b3723b6e447", "uri": "../flows/59a9181c-3aaf-46ee-8b13-2b3723b6e447.xml"}, "exchange direction": "OUTPUT", "other": {"anies": [{"name": "referenceToUnitGroupDataSet", "value": {"shortDescription": [{"value": "kg", "lang": "en"}], "type": "unit group data set", "refObjectId": "ad38d542-3fe9-439d-9b95-2f5f7752acaf", "uri": "../unitgroups/ad38d542-3fe9-439d-9b95-2f5f7752acaf.xml"}}, {"value": "0", "module": "A1-A3"}, {"value": "0", "module": "A4"}, {"value": "0", "module": "A5"}, {"value": "0", "module": "B1"}, {"value": "0", "module": "C1"}, {"value": "0", "module": "C2"}, {"value": "0", "module": "C3"}, {"value": "0", "module": "C4"}, {"value": "0", "module": "D", "scenario": "S1"}, {"value": "0", "module": "D", "scenario": "S2"}]}, "resolvedFlowVersion": "38.00.000", "flowProperties": [], "typeOfFlow": "Other flow", "classification": {"classHierarchy": "Quantities / Environmental quantities / EPD EN 15804 / LCI indicators", "name": "GaBiCategories"}}, {"dataSetInternalID": 17, "referenceToFlowDataSet": {"shortDescription": [{"value": "Exported electrical energy (EEE)", "lang": "en"}, {"value": "Exportierte elektrische Energie (EEE)", "lang": "de"}], "type": "flow data set", "refObjectId": "4da0c987-2b76-40d6-9e9e-82a017aaaf29", "uri": "../flows/4da0c987-2b76-40d6-9e9e-82a017aaaf29.xml"}, "exchange direction": "OUTPUT", "other": {"anies": [{"name": "referenceToUnitGroupDataSet", "value": {"shortDescription": [{"value": "MJ", "lang": "en"}], "type": "unit group data set", "refObjectId": "93a60a57-a3c8-11da-a746-0800200c9a66", "uri": "../unitgroups/93a60a57-a3c8-11da-a746-0800200c9a66.xml"}}, {"value": "0", "module": "A1-A3"}, {"value": "0", "module": "A4"}, {"value": "0", "module": "A5"}, {"value": "0", "module": "B1"}, {"value": "0", "module": "C1"}, {"value": "0", "module": "C2"}, {"value": "0", "module": "C3"}, {"value": "0", "module": "C4"}, {"value": "0", "module": "D", "scenario": "S1"}, {"value": "0", "module": "D", "scenario": "S2"}]}, "resolvedFlowVersion": "38.00.000", "flowProperties": [], "typeOfFlow": "Other flow", "classification": {"classHierarchy": "Quantities / Environmental quantities / EPD EN 15804 / LCI indicators", "name": "GaBiCategories"}}, {"dataSetInternalID": 18, "referenceToFlowDataSet": {"shortDescription": [{"value": "Exported thermal energy (EET)", "lang": "en"}, {"value": "Exportierte thermische Energie (EET)", "lang": "de"}], "type": "flow data set", "refObjectId": "98daf38a-7a79-46d3-9a37-2b7bd0955810", "uri": "../flows/98daf38a-7a79-46d3-9a37-2b7bd0955810.xml"}, "exchange direction": "OUTPUT", "other": {"anies": [{"name": "referenceToUnitGroupDataSet", "value": {"shortDescription": [{"value": "MJ", "lang": "en"}], "type": "unit group data set", "refObjectId": "93a60a57-a3c8-11da-a746-0800200c9a66", "uri": "../unitgroups/93a60a57-a3c8-11da-a746-0800200c9a66.xml"}}, {"value": "0", "module": "A1-A3"}, {"value": "0", "module": "A4"}, {"value": "0", "module": "A5"}, {"value": "0", "module": "B1"}, {"value": "0", "module": "C1"}, {"value": "0", "module": "C2"}, {"value": "0", "module": "C3"}, {"value": "0", "module": "C4"}, {"value": "0", "module": "D", "scenario": "S1"}, {"value": "0", "module": "D", "scenario": "S2"}]}, "resolvedFlowVersion": "38.00.000", "flowProperties": [], "typeOfFlow": "Other flow", "classification": {"classHierarchy": "Quantities / Environmental quantities / EPD EN 15804 / LCI indicators", "name": "GaBiCategories"}}]}, "LCIAResults": {"LCIAResult": [{"referenceToLCIAMethodDataSet": {"shortDescription": [{"value": "Global Warming Potential total (GWP-total)", "lang": "en"}, {"value": "Globales Erwärmungspotenzial total (GWP-total)", "lang": "de"}], "type": "LCIA method data set", "refObjectId": "6a37f984-a4b3-458a-a20a-64418c145fa2", "uri": "../lciamethods/6a37f984-a4b3-458a-a20a-64418c145fa2.xml"}, "other": {"anies": [{"name": "referenceToUnitGroupDataSet", "value": {"shortDescription": [{"value": "kg CO_(2)-Äq.", "lang": "en"}], "type": "unit group data set", "refObjectId": "1ebf3012-d0db-4de2-aefd-ef30cedb0be1", "uri": "../unitgroups/1ebf3012-d0db-4de2-aefd-ef30cedb0be1.xml"}}, {"value": "40.6884752220227", "module": "A1-A3"}, {"value": "4.9548791140375", "module": "A4"}, {"value": "0.0673798414662357", "module": "A5"}, {"value": "-19.9019", "module": "B1"}, {"value": "0.395793839816477", "module": "C1"}, {"value": "0.976599120986366", "module": "C2"}, {"value": "0.877466090215959", "module": "C3"}, {"value": "0.508875055596515", "module": "C4"}, {"value": "0", "module": "D", "scenario": "S1"}, {"value": "-2.65909558148477", "module": "D", "scenario": "S2"}]}}, {"referenceToLCIAMethodDataSet": {"shortDescription": [{"value": "Global Warming Potential fossil fuels (GWP-fossil)", "lang": "en"}, {"value": "Globales Erwärmungspotenzial fossil (GWP-fossil)", "lang": "de"}], "type": "LCIA method data set", "refObjectId": "5f635281-343e-44fb-83df-1971b155e6b6", "uri": "../lciamethods/5f635281-343e-44fb-83df-1971b155e6b6.xml"}, "other": {"anies": [{"name": "referenceToUnitGroupDataSet", "value": {"shortDescription": [{"value": "kg CO_(2)-Äq.", "lang": "en"}], "type": "unit group data set", "refObjectId": "1ebf3012-d0db-4de2-aefd-ef30cedb0be1", "uri": "../unitgroups/1ebf3012-d0db-4de2-aefd-ef30cedb0be1.xml"}}, {"value": "40.6794572571462", "module": "A1-A3"}, {"value": "4.95289833871673", "module": "A4"}, {"value": "0.0673778228612161", "module": "A5"}, {"value": "-19.9019", "module": "B1"}, {"value": "0.39575434282774", "module": "C1"}, {"value": "0.976208713189805", "module": "C2"}, {"value": "0.877235128563961", "module": "C3"}, {"value": "0.508760609404632", "module": "C4"}, {"value": "0", "module": "D", "scenario": "S1"}, {"value": "-2.65510228637502", "module": "D", "scenario": "S2"}]}}, {"referenceToLCIAMethodDataSet": {"shortDescription": [{"value": "Global Warming Potential biogenic (GWP-biogenic)", "lang": "en"}, {"value": "Globales Erwärmungspotenzial biogen (GWP-biogenic)", "lang": "de"}], "type": "LCIA method data set", "refObjectId": "2356e1ab-0185-4db5-86e5-16de51c7485c", "uri": "../lciamethods/2356e1ab-0185-4db5-86e5-16de51c7485c.xml"}, "other": {"anies": [{"name": "referenceToUnitGroupDataSet", "value": {"shortDescription": [{"value": "kg CO_(2)-Äq.", "lang": "en"}], "type": "unit group data set", "refObjectId": "1ebf3012-d0db-4de2-aefd-ef30cedb0be1", "uri": "../unitgroups/1ebf3012-d0db-4de2-aefd-ef30cedb0be1.xml"}}, {"value": "0", "module": "A1-A3"}, {"value": "0", "module": "A4"}, {"value": "0", "module": "A5"}, {"value": "0", "module": "B1"}, {"value": "0", "module": "C1"}, {"value": "0", "module": "C2"}, {"value": "0", "module": "C3"}, {"value": "0", "module": "C4"}, {"value": "0", "module": "D", "scenario": "S1"}, {"value": "0", "module": "D", "scenario": "S2"}]}}, {"referenceToLCIAMethodDataSet": {"shortDescription": [{"value": "Global Warming Potential luluc (GWP-luluc)", "lang": "en"}, {"value": "Globales Erwärmungspotenzial luluc (GWP-luluc)", "lang": "de"}], "type": "LCIA method data set", "refObjectId": "4331bbdb-978a-490d-8707-eeb047f01a55", "uri": "../lciamethods/4331bbdb-978a-490d-8707-eeb047f01a55.xml"}, "other": {"anies": [{"name": "referenceToUnitGroupDataSet", "value": {"shortDescription": [{"value": "kg CO_(2)-Äq.", "lang": "en"}], "type": "unit group data set", "refObjectId": "1ebf3012-d0db-4de2-aefd-ef30cedb0be1", "uri": "../unitgroups/1ebf3012-d0db-4de2-aefd-ef30cedb0be1.xml"}}, {"value": "0.00901796487654196", "module": "A1-A3"}, {"value": "0.00198077532077274", "module": "A4"}, {"value": "2.0186050196372E-06", "module": "A5"}, {"value": "0", "module": "B1"}, {"value": "3.94969887368684E-05", "module": "C1"}, {"value": "0.000390407796561128", "module": "C2"}, {"value": "0.000230961651998361", "module": "C3"}, {"value": "0.000114446191882876", "module": "C4"}, {"value": "0", "module": "D", "scenario": "S1"}, {"value": "-0.00399329510974712", "module": "D", "scenario": "S2"}]}}, {"referenceToLCIAMethodDataSet": {"shortDescription": [{"value": "Depletion potential of the stratospheric ozone layer (ODP)", "lang": "en"}, {"value": "Abbau Potential der stratosphärischen Ozonschicht (ODP)", "lang": "de"}], "type": "LCIA method data set", "refObjectId": "b5c629d6-def3-11e6-bf01-fe55135034f3", "uri": "../lciamethods/b5c629d6-def3-11e6-bf01-fe55135034f3.xml"}, "other": {"anies": [{"name": "referenceToUnitGroupDataSet", "value": {"shortDescription": [{"value": "kg CFC11-Äq.", "lang": "en"}], "type": "unit group data set", "refObjectId": "d9e957c9-7309-4474-bf3a-7777df6c4e5b", "uri": "../unitgroups/d9e957c9-7309-4474-bf3a-7777df6c4e5b.xml"}}, {"value": "2.05961424774714E-06", "module": "A1-A3"}, {"value": "1.14777763344932E-06", "module": "A4"}, {"value": "7.66547529938196E-10", "module": "A5"}, {"value": "0", "module": "B1"}, {"value": "8.45896996469312E-08", "module": "C1"}, {"value": "2.26225222072275E-07", "module": "C2"}, {"value": "1.91173312688858E-07", "module": "C3"}, {"value": "2.51845111411309E-07", "module": "C4"}, {"value": "0", "module": "D", "scenario": "S1"}, {"value": "-1.73300760134586E-07", "module": "D", "scenario": "S2"}]}}, {"referenceToLCIAMethodDataSet": {"shortDescription": [{"value": "Acidification potential of land and water (AP)", "lang": "en"}, {"value": "Versauerungspotenzial von Boden und Wasser (AP)", "lang": "de"}], "type": "LCIA method data set", "refObjectId": "b5c611c6-def3-11e6-bf01-fe55135034f3", "uri": "../lciamethods/b5c611c6-def3-11e6-bf01-fe55135034f3.xml"}, "other": {"anies": [{"name": "referenceToUnitGroupDataSet", "value": {"shortDescription": [{"value": "mol H^(+)-Äq.", "lang": "en"}], "type": "unit group data set", "refObjectId": "42e089ac-92bf-4bf2-8ca1-5fc40d18f2ed", "uri": "../unitgroups/42e089ac-92bf-4bf2-8ca1-5fc40d18f2ed.xml"}}, {"value": "0.0861374228825176", "module": "A1-A3"}, {"value": "0.014065549838418", "module": "A4"}, {"value": "4.05549373224631E-05", "module": "A5"}, {"value": "0", "module": "B1"}, {"value": "0.00411167567194924", "module": "C1"}, {"value": "0.00277229843397648", "module": "C2"}, {"value": "0.0073963692701797", "module": "C3"}, {"value": "0.00499010911515111", "module": "C4"}, {"value": "0", "module": "D", "scenario": "S1"}, {"value": "-0.0217857423920818", "module": "D", "scenario": "S2"}]}}, {"referenceToLCIAMethodDataSet": {"shortDescription": [{"value": "Eutrophication potential aquatic freshwater (EP-freshwater)", "lang": "en"}, {"value": "Eutrophierungspotenzial Süßwasser (EP-freshwater)", "lang": "de"}], "type": "LCIA method data set", "refObjectId": "b53ec18f-7377-4ad3-86eb-cc3f4f276b2b", "uri": "../lciamethods/b53ec18f-7377-4ad3-86eb-cc3f4f276b2b.xml"}, "other": {"anies": [{"name": "referenceToUnitGroupDataSet", "value": {"shortDescription": [{"value": "kg PO_(4)-Äq.", "lang": "en"}], "type": "unit group data set", "refObjectId": "0429039d-a61d-4590-ba67-aa4a20a810a1", "uri": "../unitgroups/0429039d-a61d-4590-ba67-aa4a20a810a1.xml"}}, {"value": "0.00142063218627533", "module": "A1-A3"}, {"value": "3.5319197122992E-05", "module": "A4"}, {"value": "6.04245968435397E-08", "module": "A5"}, {"value": "0", "module": "B1"}, {"value": "1.31201676084151E-06", "module": "C1"}, {"value": "6.9613599182547E-06", "module": "C2"}, {"value": "5.87279722024627E-06", "module": "C3"}, {"value": "3.23891194471105E-06", "module": "C4"}, {"value": "0", "module": "D", "scenario": "S1"}, {"value": "-0.00019979828351098", "module": "D", "scenario": "S2"}]}}, {"referenceToLCIAMethodDataSet": {"shortDescription": [{"value": "Eutrophication potential aquatic marine (EP-marine)", "lang": "en"}, {"value": "Eutrophierungspotenzial Salzwasser (EP-marine)", "lang": "de"}], "type": "LCIA method data set", "refObjectId": "b5c619fa-def3-11e6-bf01-fe55135034f3", "uri": "../lciamethods/b5c619fa-def3-11e6-bf01-fe55135034f3.xml"}, "other": {"anies": [{"name": "referenceToUnitGroupDataSet", "value": {"shortDescription": [{"value": "kg N-Äq.", "lang": "en"}], "type": "unit group data set", "refObjectId": "d05bb823-ecdf-4686-8c40-bf1d9257859f", "uri": "../unitgroups/d05bb823-ecdf-4686-8c40-bf1d9257859f.xml"}}, {"value": "0.0104063173224537", "module": "A1-A3"}, {"value": "0.00279519287788357", "module": "A4"}, {"value": "1.72465830162816E-05", "module": "A5"}, {"value": "0", "module": "B1"}, {"value": "0.00181955869809259", "module": "C1"}, {"value": "0.00055092825570553", "module": "C2"}, {"value": "0.00305367733385547", "module": "C3"}, {"value": "0.00188037469870885", "module": "C4"}, {"value": "0", "module": "D", "scenario": "S1"}, {"value": "-0.00423445201200214", "module": "D", "scenario": "S2"}]}}, {"referenceToLCIAMethodDataSet": {"shortDescription": [{"value": "Eutrophication potential terrestrial (EP-terrestrial)", "lang": "en"}, {"value": "Eutrophierungspotenzial Land (EP-terrestrial)", "lang": "de"}], "type": "LCIA method data set", "refObjectId": "b5c614d2-def3-11e6-bf01-fe55135034f3", "uri": "../lciamethods/b5c614d2-def3-11e6-bf01-fe55135034f3.xml"}, "other": {"anies": [{"name": "referenceToUnitGroupDataSet", "value": {"shortDescription": [{"value": "mol N-Äq.", "lang": "en"}], "type": "unit group data set", "refObjectId": "71b4d617-0ec9-4d3f-b65e-e438940c2401", "uri": "../unitgroups/71b4d617-0ec9-4d3f-b65e-e438940c2401.xml"}}, {"value": "0.241150876493639", "module": "A1-A3"}, {"value": "0.0311563117953301", "module": "A4"}, {"value": "0.000191306552881768", "module": "A5"}, {"value": "0", "module": "B1"}, {"value": "0.019958533129384", "module": "C1"}, {"value": "0.00614086156537987", "module": "C2"}, {"value": "0.033574469237685", "module": "C3"}, {"value": "0.0206991709191843", "module": "C4"}, {"value": "0", "module": "D", "scenario": "S1"}, {"value": "-0.0545833548495695", "module": "D", "scenario": "S2"}]}}, {"referenceToLCIAMethodDataSet": {"shortDescription": [{"value": "Formation potential of tropospheric ozone photochemical oxidants (POCP)", "lang": "en"}, {"value": "Bildungspotential für troposphärisches Ozon (POCP)", "lang": "de"}], "type": "LCIA method data set", "refObjectId": "b5c610fe-def3-11e6-bf01-fe55135034f3", "uri": "../lciamethods/b5c610fe-def3-11e6-bf01-fe55135034f3.xml"}, "other": {"anies": [{"name": "referenceToUnitGroupDataSet", "value": {"shortDescription": [{"value": "kg NMVOC-Äq.", "lang": "en"}], "type": "unit group data set", "refObjectId": "d27c25f8-fbc1-44c6-b47b-4adbae4199c6", "uri": "../unitgroups/d27c25f8-fbc1-44c6-b47b-4adbae4199c6.xml"}}, {"value": "0.066819035811402", "module": "A1-A3"}, {"value": "0.0119751937082828", "module": "A4"}, {"value": "4.921854373382E-05", "module": "A5"}, {"value": "0", "module": "B1"}, {"value": "0.00548837799281889", "module": "C1"}, {"value": "0.00236029242691669", "module": "C2"}, {"value": "0.0093176709683318", "module": "C3"}, {"value": "0.00592162161266569", "module": "C4"}, {"value": "0", "module": "D", "scenario": "S1"}, {"value": "-0.0132489756826632", "module": "D", "scenario": "S2"}]}}, {"referenceToLCIAMethodDataSet": {"shortDescription": [{"value": "Abiotic depletion potential for non fossil resources (ADPE)", "lang": "en"}, {"value": "Potenzial für den abiotischen Abbau nicht fossiler Ressourcen (ADPE)", "lang": "de"}], "type": "LCIA method data set", "refObjectId": "b2ad6494-c78d-11e6-9d9d-cec0c932ce01", "uri": "../lciamethods/b2ad6494-c78d-11e6-9d9d-cec0c932ce01.xml"}, "other": {"anies": [{"name": "referenceToUnitGroupDataSet", "value": {"shortDescription": [{"value": "kg Sb-Äq.", "lang": "en"}], "type": "unit group data set", "refObjectId": "54ccd2d9-a32a-4fc2-923d-f2c8c93e89d4", "uri": "../unitgroups/54ccd2d9-a32a-4fc2-923d-f2c8c93e89d4.xml"}}, {"value": "9.27470439609316E-05", "module": "A1-A3"}, {"value": "1.75604684920236E-05", "module": "A4"}, {"value": "1.80282123342236E-08", "module": "A5"}, {"value": "0", "module": "B1"}, {"value": "2.03565381449032E-07", "module": "C1"}, {"value": "3.46114157353167E-06", "module": "C2"}, {"value": "3.11096053377919E-06", "module": "C3"}, {"value": "9.92965317977722E-07", "module": "C4"}, {"value": "0", "module": "D", "scenario": "S1"}, {"value": "-1.14382041302653E-05", "module": "D", "scenario": "S2"}]}}, {"referenceToLCIAMethodDataSet": {"shortDescription": [{"value": "Abiotic depletion potential for fossil resources (ADPF)", "lang": "en"}, {"value": "Potenzial für den abiotischen Abbau fossiler Brennstoffe (ADPF)", "lang": "de"}], "type": "LCIA method data set", "refObjectId": "b2ad6110-c78d-11e6-9d9d-cec0c932ce01", "uri": "../lciamethods/b2ad6110-c78d-11e6-9d9d-cec0c932ce01.xml"}, "other": {"anies": [{"name": "referenceToUnitGroupDataSet", "value": {"shortDescription": [{"value": "MJ", "lang": "en"}], "type": "unit group data set", "refObjectId": "93a60a57-a3c8-11da-a746-0800200c9a66", "uri": "../unitgroups/93a60a57-a3c8-11da-a746-0800200c9a66.xml"}}, {"value": "284.238769724184", "module": "A1-A3"}, {"value": "75.0962850098472", "module": "A4"}, {"value": "0.0357260734837953", "module": "A5"}, {"value": "0", "module": "B1"}, {"value": "5.42907828924817", "module": "C1"}, {"value": "14.8013633112025", "module": "C2"}, {"value": "13.9110701372966", "module": "C3"}, {"value": "16.4724162198428", "module": "C4"}, {"value": "0", "module": "D", "scenario": "S1"}, {"value": "-43.9814568645236", "module": "D", "scenario": "S2"}]}}, {"referenceToLCIAMethodDataSet": {"shortDescription": [{"value": "Water use (WDP)", "lang": "en"}, {"value": "Wassernutzung (WDP)", "lang": "de"}], "type": "LCIA method data set", "refObjectId": "b2ad66ce-c78d-11e6-9d9d-cec0c932ce01", "uri": "../lciamethods/b2ad66ce-c78d-11e6-9d9d-cec0c932ce01.xml"}, "other": {"anies": [{"name": "referenceToUnitGroupDataSet", "value": {"shortDescription": [{"value": "m^(3) world-Äq. deprived", "lang": "en"}], "type": "unit group data set", "refObjectId": "6ae2df01-888e-46c8-b17d-49fa3869b476", "uri": "../unitgroups/6ae2df01-888e-46c8-b17d-49fa3869b476.xml"}}, {"value": "8.27011478757643", "module": "A1-A3"}, {"value": "0.22858151594821", "module": "A4"}, {"value": "0.00107121381360848", "module": "A5"}, {"value": "0", "module": "B1"}, {"value": "0.00849492558743106", "module": "C1"}, {"value": "0.0450530683818947", "module": "C2"}, {"value": "0.0438552780306636", "module": "C3"}, {"value": "0.0520772006859489", "module": "C4"}, {"value": "0", "module": "D", "scenario": "S1"}, {"value": "-5.06622529558526", "module": "D", "scenario": "S2"}]}}, {"referenceToLCIAMethodDataSet": {"shortDescription": [{"value": "Incidence of disease due to PM emissions (PM)", "lang": "en"}, {"value": "Auftreten von Krankheiten aufgrund von Feinstaubemissionen (PM)", "lang": "de"}], "type": "LCIA method data set", "refObjectId": "b5c602c6-def3-11e6-bf01-fe55135034f3", "uri": "../lciamethods/b5c602c6-def3-11e6-bf01-fe55135034f3.xml"}, "other": {"anies": [{"name": "referenceToUnitGroupDataSet", "value": {"shortDescription": [{"value": "Disease incidence", "lang": "en"}], "type": "unit group data set", "refObjectId": "3883559b-648f-4afc-8ba2-0bd24f3affa3", "uri": "../unitgroups/3883559b-648f-4afc-8ba2-0bd24f3affa3.xml"}}, {"value": "1.18828187568089E-06", "module": "A1-A3"}, {"value": "3.12789450745616E-07", "module": "A4"}, {"value": "2.97282043194126E-10", "module": "A5"}, {"value": "0", "module": "B1"}, {"value": "5.83646946877962E-07", "module": "C1"}, {"value": "6.16503239779473E-08", "module": "C2"}, {"value": "6.45799643189281E-07", "module": "C3"}, {"value": "1.0825009644424E-07", "module": "C4"}, {"value": "0", "module": "D", "scenario": "S1"}, {"value": "-1.81868173701187E-07", "module": "D", "scenario": "S2"}]}}, {"referenceToLCIAMethodDataSet": {"shortDescription": [{"value": "Human exposure efficiency relative to U235 (IR)", "lang": "en"}, {"value": "Wirkung durch Exposition des Menschen mit U235 (IR)", "lang": "de"}], "type": "LCIA method data set", "refObjectId": "b5c632be-def3-11e6-bf01-fe55135034f3", "uri": "../lciamethods/b5c632be-def3-11e6-bf01-fe55135034f3.xml"}, "other": {"anies": [{"name": "referenceToUnitGroupDataSet", "value": {"shortDescription": [{"value": "kBq U235-Äq.", "lang": "en"}], "type": "unit group data set", "refObjectId": "456b05bf-1415-44a9-9993-02452f554c09", "uri": "../unitgroups/456b05bf-1415-44a9-9993-02452f554c09.xml"}}, {"value": "105.287157302448", "module": "A1-A3"}, {"value": "0.32604194014636", "module": "A4"}, {"value": "0.000125709314302073", "module": "A5"}, {"value": "0", "module": "B1"}, {"value": "0.0231288370190232", "module": "C1"}, {"value": "0.0642623694389517", "module": "C2"}, {"value": "0.0924646539204124", "module": "C3"}, {"value": "0.0707274964459599", "module": "C4"}, {"value": "0", "module": "D", "scenario": "S1"}, {"value": "-0.315456910254006", "module": "D", "scenario": "S2"}]}}, {"referenceToLCIAMethodDataSet": {"shortDescription": [{"value": "Comparative toxic unit for ecosystems (ETP-fw)", "lang": "en"}, {"value": "Toxizitätsvergleichseinheit für Ökosysteme (ETP-fw)", "lang": "de"}], "type": "LCIA method data set", "refObjectId": "ee1082d1-b0f7-43ca-a1f0-21e2a4a74511", "uri": "../lciamethods/ee1082d1-b0f7-43ca-a1f0-21e2a4a74511.xml"}, "other": {"anies": [{"name": "referenceToUnitGroupDataSet", "value": {"shortDescription": [{"value": "CTUe", "lang": "en"}], "type": "unit group data set", "refObjectId": "aa959ded-f1eb-4efb-9c5c-2d60be36b3e6", "uri": "../unitgroups/aa959ded-f1eb-4efb-9c5c-2d60be36b3e6.xml"}}, {"value": "1371.52972958112", "module": "A1-A3"}, {"value": "58.9428526913203", "module": "A4"}, {"value": "0.201774118533236", "module": "A5"}, {"value": "0", "module": "B1"}, {"value": "3.1763537657718", "module": "C1"}, {"value": "11.617546422816", "module": "C2"}, {"value": "9.45040672376881", "module": "C3"}, {"value": "9.1240724014771", "module": "C4"}, {"value": "0", "module": "D", "scenario": "S1"}, {"value": "-306.129900209666", "module": "D", "scenario": "S2"}]}}, {"referenceToLCIAMethodDataSet": {"shortDescription": [{"value": "Comparative toxic unit for humans (carcinogenic) (HTP-c)", "lang": "en"}, {"value": "Toxizitätsvergleichseinheit für Menschen (krebserregend) (HTP-c)", "lang": "de"}], "type": "LCIA method data set", "refObjectId": "2299222a-bbd8-474f-9d4f-4dd1f18aea7c", "uri": "../lciamethods/2299222a-bbd8-474f-9d4f-4dd1f18aea7c.xml"}, "other": {"anies": [{"name": "referenceToUnitGroupDataSet", "value": {"shortDescription": [{"value": "CTUh", "lang": "en"}], "type": "unit group data set", "refObjectId": "d4c9523e-2d7e-49fd-8469-998f547d3a70", "uri": "../unitgroups/d4c9523e-2d7e-49fd-8469-998f547d3a70.xml"}}, {"value": "3.20065754837507E-08", "module": "A1-A3"}, {"value": "1.89571229118382E-09", "module": "A4"}, {"value": "2.64054432456805E-11", "module": "A5"}, {"value": "0", "module": "B1"}, {"value": "1.22879646965164E-10", "module": "C1"}, {"value": "3.73642003085032E-10", "module": "C2"}, {"value": "4.33909750885804E-10", "module": "C3"}, {"value": "2.08202435630296E-10", "module": "C4"}, {"value": "0", "module": "D", "scenario": "S1"}, {"value": "-1.34541044167809E-09", "module": "D", "scenario": "S2"}]}}, {"referenceToLCIAMethodDataSet": {"shortDescription": [{"value": "Comparative toxic unit for humans (noncarcinogenic) (HTP-nc)", "lang": "en"}, {"value": "Toxizitätsvergleichseinheit für Menschen (nicht krebserregend) (HTP-nc)", "lang": "de"}], "type": "LCIA method data set", "refObjectId": "3af763a5-b7a1-48c9-9cee-1f223481fcef", "uri": "../lciamethods/3af763a5-b7a1-48c9-9cee-1f223481fcef.xml"}, "other": {"anies": [{"name": "referenceToUnitGroupDataSet", "value": {"shortDescription": [{"value": "CTUh", "lang": "en"}], "type": "unit group data set", "refObjectId": "d4c9523e-2d7e-49fd-8469-998f547d3a70", "uri": "../unitgroups/d4c9523e-2d7e-49fd-8469-998f547d3a70.xml"}}, {"value": "1.23490416861336E-06", "module": "A1-A3"}, {"value": "5.95614061806592E-08", "module": "A4"}, {"value": "2.27251750391938E-10", "module": "A5"}, {"value": "0", "module": "B1"}, {"value": "2.30348697077099E-09", "module": "C1"}, {"value": "1.17394623727451E-08", "module": "C2"}, {"value": "9.0511500067591E-09", "module": "C3"}, {"value": "4.31547499716961E-09", "module": "C4"}, {"value": "0", "module": "D", "scenario": "S1"}, {"value": "-3.31173967846642E-08", "module": "D", "scenario": "S2"}]}}, {"referenceToLCIAMethodDataSet": {"shortDescription": [{"value": "Soil quality index (SQP)", "lang": "en"}, {"value": "Bodenqualitätsindex (SQP)", "lang": "de"}], "type": "LCIA method data set", "refObjectId": "b2ad6890-c78d-11e6-9d9d-cec0c932ce01", "uri": "../lciamethods/b2ad6890-c78d-11e6-9d9d-cec0c932ce01.xml"}, "other": {"anies": [{"name": "referenceToUnitGroupDataSet", "value": {"shortDescription": [{"value": "SQP", "lang": "en"}], "type": "unit group data set", "refObjectId": "f130951c-e67f-4f7f-8dd4-665de3974e18", "uri": "../unitgroups/f130951c-e67f-4f7f-8dd4-665de3974e18.xml"}}, {"value": "146.566468900716", "module": "A1-A3"}, {"value": "52.3416811660611", "module": "A4"}, {"value": "0.0149437170385597", "module": "A5"}, {"value": "0", "module": "B1"}, {"value": "0.6913101501169", "module": "C1"}, {"value": "10.3164655769111", "module": "C2"}, {"value": "7.49252925950058", "module": "C3"}, {"value": "36.6188396166494", "module": "C4"}, {"value": "0", "module": "D", "scenario": "S1"}, {"value": "-13.1881273261892", "module": "D", "scenario": "S2"}]}}]}, "otherAttributes": {"{http://www.indata.network/EPD/2019}epd-version": "1.2"}, "version": "1.1", "locations": "../ILCDLocations.xml"}