{"processInformation": {"dataSetInformation": {"UUID": "ff7c268e-cb61-41e0-8591-a41c937c8c9c", "name": {"baseName": [{"value": "AWASCHACHT PP", "lang": "de"}, {"value": "AWASCHACHT PP", "lang": "en"}], "functionalUnitFlowProperties": [{"lang": "de"}]}, "classificationInformation": {"classification": [{"class": [{"value": "Kunststoffe", "level": 0, "classId": "6"}, {"value": "Rohre", "level": 1, "classId": "6.1"}, {"value": "Abwasserrohre", "level": 2, "classId": "6.1.02"}], "name": "OEKOBAU.DAT"}, {"class": [{"value": "03 Gebäudetechnik", "level": 0}, {"value": "Anlagen zur Wasserversorgung und -entsorgung", "level": 1}, {"value": "Schächte aus Kunststoff für erdverlegte drucklose Abwasserrohrsysteme", "level": 2}], "name": "IBUCategories"}]}, "generalComment": [{"value": "Die EPD gilt fr die Kanalschachtsysteme:\nAWASCHACHT PP DN 600\nAWASCHACHT PP DN 800\nAWASCHACHT PP DN 1000\nEs handelt sich um Kanalschachtsysteme aus fllstofffreiem Polypropylen (PP). Die Systeme bestehen jeweils aus einem Schachtboden, einem Konus und optional aus einem oder mehreren Schachtringen. Zwischen den Elementen werden Dichtungen verbaut und fr den Einstieg stehen einbaubare Steigsprossen zu Verfgung. Beide Elemente sind ebenfalls Teil der Deklaration.", "lang": "de"}, {"value": "This EPD covers the sewer manhole systems:\n\nAWASCHACHT PP DN 600 \nAWASCHACHT PP DN 800 \nAWASCHACHT PP DN 1000\nThese sewer manhole systems are made from filler-free polypropylene (PP). Each system consists of a manhole floor, a cone, and one or more optional manhole rings. Seals are fitted between elements, and rungs can be installed to enable access. Both elements are covered by the declaration.", "lang": "en"}], "other": {"anies": [{"scenario": [{"description": [{"value": "100% Recycling", "lang": "de"}, {"value": "100% Recycling", "lang": "en"}], "name": "S1", "default": true}, {"description": [{"value": "100% Energetische Verwertung", "lang": "de"}, {"value": "100% Energy recovery", "lang": "en"}], "name": "S2"}, {"description": [{"value": "100% Deponierung", "lang": "de"}, {"value": "100% Landfill", "lang": "en"}], "name": "S3"}]}]}}, "quantitativeReference": {"referenceToReferenceFlow": [0]}, "time": {"referenceYear": 2024, "dataSetValidUntil": 2029, "other": {"anies": [{"name": "publicationDateOfEPD", "value": 1722902400000}]}}, "geography": {"locationOfOperationSupplyOrProduction": {"location": "DE"}}, "technology": {"technologyDescriptionAndIncludedProcesses": [{"value": "AWASCHACHT PP ist ein Kanalschachtsystem in Nennweiten zwischen DN 600 und DN 1000. Das System besteht aus einem Schachtboden, einem Konus und optional einem oder mehreren Schachtringen. Die Komponenten werden im Spritzgussverfahren hergestellt und bestehen zum Hauptteil aus Polypropylen (PP). Zwischen den Komponenten werden Dichtungen eingesetzt und zusätzliche Steigsprossen dienen dem Einstieg in den Kanalschacht. \nTechnische Daten: \nDie technischen Daten der Produkte, die im Geltungsbereich der EPD liegen, sind unter Verweis auf die den einzelnen Daten zugrundeliegenden Prfregeln genannt.\nDie Schachtsysteme AWASCHACHT PP erfllen die relevanten Normen EN 13598-2 und EN 476. \nDeklarierte Einheit: \nAls deklarierte Einheit wird \"1 kg Kanalschachtsystem ohne Produktverpackung\" verwendet, das die Komponenten Konus, Schachtring und -boden sowie Dichtungen und Steigsprossen umfasst. Eine massenanteilige Aufteilung der Komponenten ist in 2.5 dargestellt. Die Produktverpackung wird separat zum Produkt betrachtet und ist ebenfalls Teil der kobilanz.\n\nFr die LCA wurde eine Durchschnittsvariante des Kanalschachts AWASCHACHT PP bilanziert. Diese basiert auf den Verkaufsmengen fr das Bezugsjahr 2022 und deckt damit alle Produktvarianten (gelistet in 2.1) ab. Der zugehrige Massebezug unterscheidet sich je nach Nennweite und verwendeten Komponenten im Schachtsystem.", "lang": "de"}, {"value": "AWASCHACHT PP ist ein Kanalschachtsystem in Nennweiten zwischen DN 600 und DN 1000. Das System besteht aus einem Schachtboden, einem Konus und optional einem oder mehreren Schachtringen. Die Komponenten werden im Spritzgussverfahren hergestellt und bestehen zum Hauptteil aus Polypropylen (PP). Zwischen den Komponenten werden Dichtungen eingesetzt und zusätzliche Steigsprossen dienen dem Einstieg in den Kanalschacht. \nTechnical data: \nThe technical data of the products covered by this EPD are given with reference to the assessment rules underlying the individual data.\n\nThe AWASCHAFT PP manhole systems satisfy the relevant standards EN 13598-2 and EN 476. \nDeclared unit: \nThe declared unit is '1 kg sewer manhole system without product packaging', encompassing the components cone, manhole ring, manhole floor, seals, and rungs. 2.5 shows the mass fractions of the single components. The product packaging is considered separately from the product and is also included in the life-cycle assessment.\n\nAn average variant of the AWASCHACHT PP sewer manholewas assessed for the LCA. This is based on the quantities sold in the reference year 2022 and thus covers all product variants (see 2.1). The corresponding unit mass is subject to the nominal diameter and components used in the manholesystem.", "lang": "en"}], "technologicalApplicability": [{"value": "Das Schachtsystem AWASCHACHT PP wird fr Kanalsysteme im Tiefbau eingesetzt. Das Schachtsystem wird angewandt zur Leitung von Schmutz-, Misch- und Regenwasser. Zudem sind die Schchte je nach Ausfhrung besteigbar, dienen somit als Einstiegspunkt in das Kanalsystem und bieten die Mglichkeit der Inspektion und Reinigung des Kanals.", "lang": "de"}, {"value": "The AWASCHACHT PP manhole system is used for sewer systems in underground engineering. The manhole system is used to rout waste, mixed, and rain water. In addition, since the manholes are ascendable depending on design variant, they double as an access point to the sewer system and allow for inspection and cleaning of the sewer.", "lang": "en"}]}}, "modellingAndValidation": {"LCIMethodAndAllocation": {"typeOfDataSet": "EPD", "referenceToLCAMethodDetails": [{"shortDescription": [{"value": "Schächte aus Kunststoff für erdverlegte drucklose Abwasserrohrsysteme.pdf", "lang": "de"}], "type": "source data set", "refObjectId": "b08b1940-f938-443f-980a-2ba0e3e87776"}], "other": {"anies": [{"name": "subType", "value": "average dataset"}]}}, "dataSourcesTreatmentAndRepresentativeness": {"referenceToDataSource": [{"shortDescription": [{"value": "GaBi Database (all versions)", "lang": "de"}], "type": "source data set", "refObjectId": "28d74cc0-db8b-4d7e-bc44-5f6d56ce0c4a"}, {"shortDescription": [{"value": "Sphera MLC (fka GaBi) CUP 2023.02", "lang": "de"}], "type": "source data set", "refObjectId": "cb600d3b-e85a-42b3-b059-5591e2757fbb"}], "useAdviceForDataSet": [{"value": "Gültigkeitsbereich: \nDie EPD gilt fr die Kanalschachtsysteme\nAWASCHACHT PP DN 600\nAWASCHACHT PP DN 800\nAWASCHACHT PP DN 1000hergestellt im\nREHAU-Werk Viechtach, Deutschlandder Firma\nREHAU Industries SE & Co. KG.\nDie Herstellung der Kanalschachtsysteme erfolgt in Deutschland. Die Produkte werden weltweit verwendet, mit dem Fokus auf Europa.\n\nEs handelt sich um eine Durchschnitts-EPD, bei der die oben genannten Produkte ber eine durchschnittliche Produktvariante deklariert werden. \nSystemgrenze: \nEs wird der gesamte Produktlebenszyklus von AWASCHACHT PP betrachtet – siehe Flieschema.\nTyp der EPD: Wiege bis Bahre (Module A, B, C, D).\n\nDas nachfolgende Flieschema zeigt die Systemgrenzen bei der Bilanzierung von AWASCHACHT PP:\n\n\nIm Folgenden sind die bercksichtigten Lebenswegabschnitte bzw. Prozessmodule fr die Herstellung der Kanalschachtsysteme detailliert aufgelistet:\n\nA1–A3 Herstellungsphase\nProduktion der Roh-, Hilfs- und Betriebsstoffe sowie der Vorprodukte inkl. Transport zum jeweiligen Werk\nEnergiebereitstellung fr die Produktion\nProduktion und Verpackung des Kanalschachtsystems im Werk Viechtach\nExterne Wiederaufbereitung der Produktionsabflle und Rckfhrung in Produktion\nVerwertung weiterer Abflle inkl. Transport\nA4–A5 Aufbauphase\nTransport des Produkts zur Baustelle\nEinbau des Kanalschachts\nVerwertung der Produktverpackung\nB Nutzungsphase\nNutzung des Kanalschachtsystems (B1)\nInstandhaltung des Kanalschachtsystems (B2)\nBetrieblicher Energie- und Wassereinsatz (B6, B7)\nC1–C4 Entsorgung\nEs werden drei 100-%-Entsorgungsszenarien angenommen:\nEnd-of-Life (EoL) Szenario 1: 100 % Rckbau des Kanalschachts mit anschlieender werkstofflicher Verwertung (Modul C3/1 und D/1 in der Auswertung).\nEoL-Szenario 2: 100 % Rckbau des Kanalschachts mit anschlieender energetischer Verwertung (Modul C3/2 und D/2 in der Auswertung).\nEoL-Szenario 3: 100 % Rckbau des Kanalschachts und Entsorgung auf einer lokalen Deponie (Modul C4/3 in der Auswertung)\n\nD Wiederverwendungs-, Rckgewinnungs- und/oder Recyclingpotentiale\nWiederverwendungs-, Rckgewinnungs-, und/oder Recyclingpotentiale sind in den Entsorgungsszenarien vorhanden, da hier die Kanalschachtsysteme einer energetischen bzw. stofflichen Verwertung zugefhrt werden, aus denen Energie bzw. Sekundrmaterialien zurckgewonnen werden, die auerhalb der Systemgrenze genutzt werden knnen.", "lang": "de"}, {"value": "Scope: \nThis EPD covers the sewer manhole systems\n\nAWASCHACHT PP DN 600 \nAWASCHACHT PP DN 800 \nAWASCHACHT PP DN 1000 \nmanufactured at \n\nREHAU plant Viechtach, Germany, of the company \nREHAU Industries SE & Co. KG. \nThe sewer manhole systems are manufactured in Germany. The products are used worldwide, with particular focus on Europe. \n\nThis is an average EPD in which the products named above are declared on the basis of an average product variant. \nSystem boundary: \nThe entire product life cycle of AWASCHACHT PP is considered, see the flow diagram.EPD type: cradle to the grave (modules A, B, C, and D).The following flow diagram shows the system boundaries in the life-cycle assessment of AWASCHACHT PP:\n\n\nThe life cycle segments or process modules for the manufacture of the sewer manhole systems are detailed below:\n\nA1–A3 Manufacturing phase \n\nProduction of the base, auxiliary and operating materials and of the intermediate products incl. transport to factory• Energy supply for production \nProduction and packaging of the sewer manholesystem at the Viechtach factory \nInternal reprocessing of production waste and feedback into production \nRecycling of other waste incl. transport \nA4–A5 Set-up phase \nTransport of product to construction site \nInstallation of sewer manhole \nRecycling of product packaging \nB use phase \n\nDeployment of sewer manhole system (B1) \nMaintenance of sewer manhole system (B2) \nEnergy and water consumption during operation (B6, B7)\nC1–C4 Disposal \nThree 100% disposal scenarios are assumed: \n\nEnd-of-Life (EoL) scenario 1: 100% dismantling of sewer manhole and material utilisation (module C3/1 and D/1 in the evaluation). \nEoL scenario 2: 100% dismantling of sewer manholeand energetic utilisation (module C3/2 and D/2 in the evaluation). \nEoL scenario 3: 100% dismantling of sewer manholeand disposal at local landfill (module C4/3 in the evaluation) D Reuse, recovery and/or recycling potentials \n\nReuse, recovery and/or recycling potentials exist in the disposal scenarios because the sewer manhole systems are put to energetic or material utilisation with recovery of energy or secondary materials which can then be used outside the system boundary.", "lang": "en"}], "other": {"anies": [{"name": "referenceToOriginalEPD", "value": {"shortDescription": {"value": "AWASCHACHT PP.pdf", "defaultValue": "AWASCHACHT PP.pdf", "lstrings": [{"lang": "de", "value": "AWASCHACHT PP.pdf"}]}, "type": "source data set", "uuid": {"uuid": "6417d3e3-2e56-4cd2-992c-e14854552f21"}, "refObjectId": "6417d3e3-2e56-4cd2-992c-e14854552f21", "resourceURLs": ["https://oekobaudat.de/OEKOBAU.DAT/resource/sources/6417d3e3-2e56-4cd2-992c-e14854552f21/AWASCHACHT_PP_19707.pdf?version=00.01.000"]}}]}}, "validation": {"review": [{"referenceToNameOfReviewerAndInstitution": [{"shortDescription": [{"value": "Institut Bauen und Umwelt e. V.", "lang": "de"}], "type": "contact data set", "refObjectId": "d111dbec-b024-4be5-86c5-752d6eb2cf95", "uri": "../contacts/d111dbec-b024-4be5-86c5-752d6eb2cf95.xml"}], "type": "Accredited third party review"}]}, "complianceDeclarations": {"compliance": [{"referenceToComplianceSystem": {"shortDescription": [{"value": "DIN EN 15804+A2", "lang": "de"}], "type": "source data set", "refObjectId": "c0016b33-8cf7-415c-ac6e-deba0d21440d", "uri": "../sources/c0016b33-8cf7-415c-ac6e-deba0d21440d.xml"}}, {"referenceToComplianceSystem": {"shortDescription": [{"value": "ISO 14025", "lang": "de"}], "type": "source data set", "refObjectId": "4f2eb655-6e44-4874-a95a-e28f5442cd4d", "uri": "../sources/4f2eb655-6e44-4874-a95a-e28f5442cd4d.xml"}}]}}, "administrativeInformation": {"commissionerAndGoal": {"referenceToCommissioner": [{"shortDescription": [{"value": "REHAU Industries SE & Co. KG", "lang": "de"}], "type": "contact data set", "refObjectId": "b1b59d51-66a3-4983-acd8-86ad04e48050", "uri": "../contacts/b1b59d51-66a3-4983-acd8-86ad04e48050.xml"}]}, "dataGenerator": {"referenceToPersonOrEntityGeneratingTheDataSet": [{"shortDescription": [{"value": "SKZ - Das Kunststoff-Zentrum", "lang": "de"}], "type": "contact data set", "refObjectId": "2da43b2d-777d-45c6-ba4b-76c55a616a00", "uri": "../contacts/2da43b2d-777d-45c6-ba4b-76c55a616a00.xml"}]}, "dataEntryBy": {"timeStamp": 1722902400000, "referenceToDataSetFormat": [{"shortDescription": [{"value": "ILCD Format", "lang": "de"}], "type": "source data set", "refObjectId": "a97a0155-0234-4b87-b4ce-a45da52f2a40", "uri": "../sources/a97a0155-0234-4b87-b4ce-a45da52f2a40.xml"}, {"shortDescription": [{"value": "EPD-Datenformaterweiterungen v1.2", "lang": "de"}, {"value": "EPD Data Format Extensions v1.2", "lang": "en"}], "type": "source data set", "refObjectId": "a29449fd-aa2f-4de8-b5d7-4b06b43c6fde", "uri": "../sources/a29449fd-aa2f-4de8-b5d7-4b06b43c6fde.xml"}]}, "publicationAndOwnership": {"dataSetVersion": "00.07.000", "referenceToRegistrationAuthority": {"shortDescription": [{"value": "Institut Bauen und Umwelt e. V.", "lang": "de"}], "type": "contact data set", "refObjectId": "d111dbec-b024-4be5-86c5-752d6eb2cf95", "uri": "../contacts/d111dbec-b024-4be5-86c5-752d6eb2cf95.xml"}, "registrationNumber": "EPD-REH-20240255-IBA1-DE", "referenceToOwnershipOfDataSet": {"shortDescription": [{"value": "REHAU Industries SE & Co. KG", "lang": "de"}], "type": "contact data set", "refObjectId": "b1b59d51-66a3-4983-acd8-86ad04e48050", "uri": "../contacts/b1b59d51-66a3-4983-acd8-86ad04e48050.xml"}, "copyright": true, "licenseType": "Free of charge for all users and uses", "accessRestrictions": [{"value": "None", "lang": "en"}], "other": {"anies": [{"name": "referenceToPublisher", "value": {"shortDescription": [{"value": "Institut Bauen und Umwelt e. V.", "lang": "de"}], "type": "contact data set", "refObjectId": "d111dbec-b024-4be5-86c5-752d6eb2cf95", "uri": "../contacts/d111dbec-b024-4be5-86c5-752d6eb2cf95.xml"}}]}}}, "exchanges": {"exchange": [{"dataSetInternalID": 0, "referenceToFlowDataSet": {"shortDescription": [{"value": "AWASCHACHT PP (AWASCHACHT PP)", "lang": "de"}], "type": "flow data set", "refObjectId": "4f811ef5-2489-ea00-99fb-ae5164342c47", "uri": "../flows/4f811ef5-2489-ea00-99fb-ae5164342c47.xml"}, "meanAmount": 1.0, "referencesToDataSource": {}, "referenceFlow": true, "resolvedFlowVersion": "00.07.000", "resultingflowAmount": 1.0, "flowProperties": [{"name": [{"lang": "en", "value": "Mass"}, {"lang": "de", "value": "Masse"}], "uuid": "93a60a56-a3c8-11da-a746-0800200b9a66", "referenceFlowProperty": true, "meanValue": 1.0, "referenceUnit": "kg", "unitGroupUUID": "ad38d542-3fe9-439d-9b95-2f5f7752acaf"}], "materialProperties": [{"name": "weight per piece", "value": "92.5", "unit": "kg"}, {"name": "gross density", "value": "900.0", "unit": "kg/m^3", "unitDescription": "kilograms per cubic metre"}], "typeOfFlow": "Product flow", "classification": {"classHierarchy": "Kunststoffe / Rohre / Abwasserrohre", "name": "OEKOBAU.DAT"}}, {"dataSetInternalID": 1, "referenceToFlowDataSet": {"shortDescription": [{"value": "Erneuerbare Primärenergie als Energieträger (PERE)", "lang": "de"}, {"value": "Renewable primary energy as energy carrier (PERE)", "lang": "en"}], "type": "flow data set", "refObjectId": "20f32be5-0398-4288-9b6d-accddd195317", "uri": "../flows/20f32be5-0398-4288-9b6d-accddd195317.xml"}, "exchange direction": "INPUT", "other": {"anies": [{"name": "referenceToUnitGroupDataSet", "value": {"shortDescription": [{"value": "MJ", "lang": "de"}], "type": "unit group data set", "refObjectId": "93a60a57-a3c8-11da-a746-0800200c9a66", "uri": "../unitgroups/93a60a57-a3c8-11da-a746-0800200c9a66.xml"}}, {"value": "11.4265097516902", "module": "A1-A3"}, {"value": "0.0370617220630755", "module": "A4"}, {"value": "0.743242249026367", "module": "A5"}, {"value": "0", "module": "B1"}, {"value": "0.120672780960171", "module": "B2"}, {"value": "0", "module": "B6"}, {"value": "0", "module": "B7"}, {"value": "0.0386558324144871", "module": "C1"}, {"value": "0.00425885772561494", "module": "C2"}, {"value": "0.0670974572368029", "module": "C3", "scenario": "S1"}, {"value": "0.102390226753187", "module": "C3", "scenario": "S2"}, {"value": "0.0926344716058196", "module": "C4"}, {"value": "-1.79719086705451", "module": "D", "scenario": "S1"}, {"value": "-5.84201885442263", "module": "D", "scenario": "S2"}, {"value": "0", "module": "D", "scenario": "S3"}]}, "resolvedFlowVersion": "38.00.000", "flowProperties": [], "typeOfFlow": "Other flow", "classification": {"classHierarchy": "Quantities", "name": "GaBiCategories"}}, {"dataSetInternalID": 2, "referenceToFlowDataSet": {"shortDescription": [{"value": "Erneuerbare Primärenergie zur stofflichen Nutzung (PERM)", "lang": "de"}, {"value": "Renewable primary energy resources as material utilization (PERM)", "lang": "en"}], "type": "flow data set", "refObjectId": "fb3ec0de-548d-4508-aea5-00b73bf6f702", "uri": "../flows/fb3ec0de-548d-4508-aea5-00b73bf6f702.xml"}, "exchange direction": "INPUT", "other": {"anies": [{"name": "referenceToUnitGroupDataSet", "value": {"shortDescription": [{"value": "MJ", "lang": "de"}], "type": "unit group data set", "refObjectId": "93a60a57-a3c8-11da-a746-0800200c9a66", "uri": "../unitgroups/93a60a57-a3c8-11da-a746-0800200c9a66.xml"}}, {"value": "0.7402462524", "module": "A1-A3"}, {"value": "0", "module": "A4"}, {"value": "-0.7327", "module": "A5"}, {"value": "0", "module": "B1"}, {"value": "0", "module": "B2"}, {"value": "0", "module": "B6"}, {"value": "0", "module": "B7"}, {"value": "0", "module": "C1"}, {"value": "0", "module": "C2"}, {"value": "-0.0075462524", "module": "C3", "scenario": "S1"}, {"value": "-0.0075462524", "module": "C3", "scenario": "S2"}, {"value": "0", "module": "C4"}, {"value": "0", "module": "D", "scenario": "S1"}, {"value": "0", "module": "D", "scenario": "S2"}, {"value": "0", "module": "D", "scenario": "S3"}]}, "resolvedFlowVersion": "38.00.000", "flowProperties": [], "typeOfFlow": "Other flow", "classification": {"classHierarchy": "Quantities", "name": "GaBiCategories"}}, {"dataSetInternalID": 3, "referenceToFlowDataSet": {"shortDescription": [{"value": "Total erneuerbare Primärenergie (PERT)", "lang": "de"}, {"value": "Total use of renewable primary energy resources (PERT)", "lang": "en"}], "type": "flow data set", "refObjectId": "53f97275-fa8a-4cdd-9024-65936002acd0", "uri": "../flows/53f97275-fa8a-4cdd-9024-65936002acd0.xml"}, "exchange direction": "INPUT", "other": {"anies": [{"name": "referenceToUnitGroupDataSet", "value": {"shortDescription": [{"value": "MJ", "lang": "de"}], "type": "unit group data set", "refObjectId": "93a60a57-a3c8-11da-a746-0800200c9a66", "uri": "../unitgroups/93a60a57-a3c8-11da-a746-0800200c9a66.xml"}}, {"value": "12.1667560040902", "module": "A1-A3"}, {"value": "0.0370617220630755", "module": "A4"}, {"value": "0.0105422490263672", "module": "A5"}, {"value": "0", "module": "B1"}, {"value": "0.120672780960171", "module": "B2"}, {"value": "0", "module": "B6"}, {"value": "0", "module": "B7"}, {"value": "0.0386558324144871", "module": "C1"}, {"value": "0.00425885772561494", "module": "C2"}, {"value": "0.0595512048368029", "module": "C3", "scenario": "S1"}, {"value": "0.0948439743531875", "module": "C3", "scenario": "S2"}, {"value": "0.0926344716058196", "module": "C4"}, {"value": "-1.79719086705451", "module": "D", "scenario": "S1"}, {"value": "-5.87381934982972E-09", "module": "D", "scenario": "S2"}, {"value": "0", "module": "D", "scenario": "S3"}]}, "resolvedFlowVersion": "38.00.000", "flowProperties": [], "typeOfFlow": "Other flow", "classification": {"classHierarchy": "Quantities / Environmental quantities / EPD EN 15804 / LCI indicators", "name": "GaBiCategories"}}, {"dataSetInternalID": 4, "referenceToFlowDataSet": {"shortDescription": [{"value": "Nicht-erneuerbare Primärenergie als Energieträger (PENRE)", "lang": "de"}, {"value": "Non renewable primary energy as energy carrier (PENRE)", "lang": "en"}], "type": "flow data set", "refObjectId": "ac857178-2b45-46ec-892a-a9a4332f0372", "uri": "../flows/ac857178-2b45-46ec-892a-a9a4332f0372.xml"}, "exchange direction": "INPUT", "other": {"anies": [{"name": "referenceToUnitGroupDataSet", "value": {"shortDescription": [{"value": "MJ", "lang": "de"}], "type": "unit group data set", "refObjectId": "93a60a57-a3c8-11da-a746-0800200c9a66", "uri": "../unitgroups/93a60a57-a3c8-11da-a746-0800200c9a66.xml"}}, {"value": "70.8631359102304", "module": "A1-A3"}, {"value": "0.553827407766244", "module": "A4"}, {"value": "0.0726328542065574", "module": "A5"}, {"value": "0", "module": "B1"}, {"value": "2.0718973622358", "module": "B2"}, {"value": "0", "module": "B6"}, {"value": "0", "module": "B7"}, {"value": "0.547375900782027", "module": "C1"}, {"value": "0.058742644963757", "module": "C2"}, {"value": "3.45349784047729", "module": "C3", "scenario": "S1"}, {"value": "42.06551902539", "module": "C3", "scenario": "S2"}, {"value": "1.0271829377317", "module": "C4"}, {"value": "-33.5921879271385", "module": "D", "scenario": "S1"}, {"value": "-26.1356769399812", "module": "D", "scenario": "S2"}, {"value": "0", "module": "D", "scenario": "S3"}]}, "resolvedFlowVersion": "38.00.000", "flowProperties": [], "typeOfFlow": "Other flow", "classification": {"classHierarchy": "Quantities", "name": "GaBiCategories"}}, {"dataSetInternalID": 5, "referenceToFlowDataSet": {"shortDescription": [{"value": "Nicht-erneuerbare Primärenergie zur stofflichen Nutzung (PENRM)", "lang": "de"}, {"value": "Non renewable primary energy as material utilization (PENRM)", "lang": "en"}], "type": "flow data set", "refObjectId": "1421caa0-679d-4bf4-b282-0eb850ccae27", "uri": "../flows/1421caa0-679d-4bf4-b282-0eb850ccae27.xml"}, "exchange direction": "INPUT", "other": {"anies": [{"name": "referenceToUnitGroupDataSet", "value": {"shortDescription": [{"value": "MJ", "lang": "de"}], "type": "unit group data set", "refObjectId": "93a60a57-a3c8-11da-a746-0800200c9a66", "uri": "../unitgroups/93a60a57-a3c8-11da-a746-0800200c9a66.xml"}}, {"value": "41.6929445237675", "module": "A1-A3"}, {"value": "0", "module": "A4"}, {"value": "0.000168079956628989", "module": "A5"}, {"value": "0", "module": "B1"}, {"value": "0", "module": "B2"}, {"value": "0", "module": "B6"}, {"value": "0", "module": "B7"}, {"value": "0", "module": "C1"}, {"value": "0", "module": "C2"}, {"value": "-41.6931126037242", "module": "C3", "scenario": "S1"}, {"value": "-41.6931126037242", "module": "C3", "scenario": "S2"}, {"value": "0", "module": "C4"}, {"value": "0", "module": "D", "scenario": "S1"}, {"value": "0", "module": "D", "scenario": "S2"}, {"value": "0", "module": "D", "scenario": "S3"}]}, "resolvedFlowVersion": "38.00.000", "flowProperties": [], "typeOfFlow": "Other flow", "classification": {"classHierarchy": "Quantities", "name": "GaBiCategories"}}, {"dataSetInternalID": 6, "referenceToFlowDataSet": {"shortDescription": [{"value": "Total nicht erneuerbare Primärenergie (PENRT)", "lang": "de"}, {"value": "Total use of non renewable primary energy resources (PENRT)", "lang": "en"}], "type": "flow data set", "refObjectId": "06159210-646b-4c8d-8583-da9b3b95a6c1", "uri": "../flows/06159210-646b-4c8d-8583-da9b3b95a6c1.xml"}, "exchange direction": "INPUT", "other": {"anies": [{"name": "referenceToUnitGroupDataSet", "value": {"shortDescription": [{"value": "MJ", "lang": "de"}], "type": "unit group data set", "refObjectId": "93a60a57-a3c8-11da-a746-0800200c9a66", "uri": "../unitgroups/93a60a57-a3c8-11da-a746-0800200c9a66.xml"}}, {"value": "112.556080433998", "module": "A1-A3"}, {"value": "0.553827407766244", "module": "A4"}, {"value": "0.0728009341631864", "module": "A5"}, {"value": "0", "module": "B1"}, {"value": "2.0718973622358", "module": "B2"}, {"value": "0", "module": "B6"}, {"value": "0", "module": "B7"}, {"value": "0.547375900782027", "module": "C1"}, {"value": "0.058742644963757", "module": "C2"}, {"value": "-38.2396147632469", "module": "C3", "scenario": "S1"}, {"value": "0.372406421665879", "module": "C3", "scenario": "S2"}, {"value": "1.0271829377317", "module": "C4"}, {"value": "-33.5921879271385", "module": "D", "scenario": "S1"}, {"value": "-26.1356769399812", "module": "D", "scenario": "S2"}, {"value": "0", "module": "D", "scenario": "S3"}]}, "resolvedFlowVersion": "38.00.000", "flowProperties": [], "typeOfFlow": "Other flow", "classification": {"classHierarchy": "Quantities / Environmental quantities / EPD EN 15804 / LCI indicators", "name": "GaBiCategories"}}, {"dataSetInternalID": 7, "referenceToFlowDataSet": {"shortDescription": [{"value": "Einsatz von Sekundärstoffen (SM)", "lang": "de"}, {"value": "Use of secondary material (SM)", "lang": "en"}], "type": "flow data set", "refObjectId": "c6a1f35f-2d09-4f54-8dfb-97e502e1ce92", "uri": "../flows/c6a1f35f-2d09-4f54-8dfb-97e502e1ce92.xml"}, "exchange direction": "INPUT", "other": {"anies": [{"name": "referenceToUnitGroupDataSet", "value": {"shortDescription": [{"value": "kg", "lang": "de"}], "type": "unit group data set", "refObjectId": "ad38d542-3fe9-439d-9b95-2f5f7752acaf", "uri": "../unitgroups/ad38d542-3fe9-439d-9b95-2f5f7752acaf.xml"}}, {"value": "0", "module": "A1-A3"}, {"value": "0", "module": "A4"}, {"value": "0", "module": "A5"}, {"value": "0", "module": "B1"}, {"value": "0", "module": "B2"}, {"value": "0", "module": "B6"}, {"value": "0", "module": "B7"}, {"value": "0", "module": "C1"}, {"value": "0", "module": "C2"}, {"value": "0", "module": "C3", "scenario": "S1"}, {"value": "0", "module": "C3", "scenario": "S2"}, {"value": "0", "module": "C4"}, {"value": "0.95", "module": "D", "scenario": "S1"}, {"value": "0", "module": "D", "scenario": "S2"}, {"value": "0", "module": "D", "scenario": "S3"}]}, "resolvedFlowVersion": "38.00.000", "flowProperties": [], "typeOfFlow": "Other flow", "classification": {"classHierarchy": "Quantities / Environmental quantities / EPD EN 15804 / LCI indicators", "name": "GaBiCategories"}}, {"dataSetInternalID": 8, "referenceToFlowDataSet": {"shortDescription": [{"value": "Erneuerbare Sekundärbrennstoffe (RSF)", "lang": "de"}, {"value": "Use of renewable secondary fuels (RSF)", "lang": "en"}], "type": "flow data set", "refObjectId": "64333088-a55f-4aa2-9a31-c10b07816787", "uri": "../flows/64333088-a55f-4aa2-9a31-c10b07816787.xml"}, "exchange direction": "INPUT", "other": {"anies": [{"name": "referenceToUnitGroupDataSet", "value": {"shortDescription": [{"value": "MJ", "lang": "de"}], "type": "unit group data set", "refObjectId": "93a60a57-a3c8-11da-a746-0800200c9a66", "uri": "../unitgroups/93a60a57-a3c8-11da-a746-0800200c9a66.xml"}}, {"value": "0", "module": "A1-A3"}, {"value": "0", "module": "A4"}, {"value": "0", "module": "A5"}, {"value": "0", "module": "B1"}, {"value": "0", "module": "B2"}, {"value": "0", "module": "B6"}, {"value": "0", "module": "B7"}, {"value": "0", "module": "C1"}, {"value": "0", "module": "C2"}, {"value": "0", "module": "C3", "scenario": "S1"}, {"value": "0", "module": "C3", "scenario": "S2"}, {"value": "0", "module": "C4"}, {"value": "0", "module": "D", "scenario": "S1"}, {"value": "0", "module": "D", "scenario": "S2"}, {"value": "0", "module": "D", "scenario": "S3"}]}, "resolvedFlowVersion": "38.00.000", "flowProperties": [], "typeOfFlow": "Other flow", "classification": {"classHierarchy": "Quantities / Environmental quantities / EPD EN 15804 / LCI indicators", "name": "GaBiCategories"}}, {"dataSetInternalID": 9, "referenceToFlowDataSet": {"shortDescription": [{"value": "Nicht erneuerbare Sekundärbrennstoffe (NRSF)", "lang": "de"}, {"value": "Use of non renewable secondary fuels (NRSF)", "lang": "en"}], "type": "flow data set", "refObjectId": "89def144-d39a-4287-b86f-efde453ddcb2", "uri": "../flows/89def144-d39a-4287-b86f-efde453ddcb2.xml"}, "exchange direction": "INPUT", "other": {"anies": [{"name": "referenceToUnitGroupDataSet", "value": {"shortDescription": [{"value": "MJ", "lang": "de"}], "type": "unit group data set", "refObjectId": "93a60a57-a3c8-11da-a746-0800200c9a66", "uri": "../unitgroups/93a60a57-a3c8-11da-a746-0800200c9a66.xml"}}, {"value": "0", "module": "A1-A3"}, {"value": "0", "module": "A4"}, {"value": "0", "module": "A5"}, {"value": "0", "module": "B1"}, {"value": "0", "module": "B2"}, {"value": "0", "module": "B6"}, {"value": "0", "module": "B7"}, {"value": "0", "module": "C1"}, {"value": "0", "module": "C2"}, {"value": "0", "module": "C3", "scenario": "S1"}, {"value": "0", "module": "C3", "scenario": "S2"}, {"value": "0", "module": "C4"}, {"value": "0", "module": "D", "scenario": "S1"}, {"value": "0", "module": "D", "scenario": "S2"}, {"value": "0", "module": "D", "scenario": "S3"}]}, "resolvedFlowVersion": "38.00.000", "flowProperties": [], "typeOfFlow": "Other flow", "classification": {"classHierarchy": "Quantities / Environmental quantities / EPD EN 15804 / LCI indicators", "name": "GaBiCategories"}}, {"dataSetInternalID": 10, "referenceToFlowDataSet": {"shortDescription": [{"value": "Einsatz von Süßwasserressourcen (FW)", "lang": "de"}, {"value": "Use of net fresh water (FW)", "lang": "en"}], "type": "flow data set", "refObjectId": "3cf952c8-f3a4-461d-8c96-96456ca62246", "uri": "../flows/3cf952c8-f3a4-461d-8c96-96456ca62246.xml"}, "exchange direction": "INPUT", "other": {"anies": [{"name": "referenceToUnitGroupDataSet", "value": {"shortDescription": [{"value": "m^3", "lang": "de"}], "type": "unit group data set", "refObjectId": "cd950537-0a98-4044-9ba7-9f9a68d0a504", "uri": "../unitgroups/cd950537-0a98-4044-9ba7-9f9a68d0a504.xml"}}, {"value": "0.00903519249332652", "module": "A1-A3"}, {"value": "3.29768079188855E-05", "module": "A4"}, {"value": "0.000212264753926741", "module": "A5"}, {"value": "0", "module": "B1"}, {"value": "0.000159701661062231", "module": "B2"}, {"value": "0", "module": "B6"}, {"value": "0", "module": "B7"}, {"value": "4.25934873004017E-05", "module": "C1"}, {"value": "4.66459704479626E-06", "module": "C2"}, {"value": "0.00202617551631989", "module": "C3", "scenario": "S1"}, {"value": "0.00676230298468199", "module": "C3", "scenario": "S2"}, {"value": "1.01281897187215E-05", "module": "C4"}, {"value": "-0.00377334417950814", "module": "D", "scenario": "S1"}, {"value": "-0.00568860009412031", "module": "D", "scenario": "S2"}, {"value": "0", "module": "D", "scenario": "S3"}]}, "resolvedFlowVersion": "38.00.000", "flowProperties": [], "typeOfFlow": "Other flow", "classification": {"classHierarchy": "Quantities / Environmental quantities / EPD EN 15804 / LCI indicators", "name": "GaBiCategories"}}, {"dataSetInternalID": 11, "referenceToFlowDataSet": {"shortDescription": [{"value": "Gefährlicher Abfall zur Deponie (HWD)", "lang": "de"}, {"value": "Hazardous waste disposed (HWD)", "lang": "en"}], "type": "flow data set", "refObjectId": "430f9e0f-59b2-46a0-8e0d-55e0e84948fc", "uri": "../flows/430f9e0f-59b2-46a0-8e0d-55e0e84948fc.xml"}, "exchange direction": "OUTPUT", "other": {"anies": [{"name": "referenceToUnitGroupDataSet", "value": {"shortDescription": [{"value": "kg", "lang": "de"}], "type": "unit group data set", "refObjectId": "ad38d542-3fe9-439d-9b95-2f5f7752acaf", "uri": "../unitgroups/ad38d542-3fe9-439d-9b95-2f5f7752acaf.xml"}}, {"value": "9.30009848608456E-09", "module": "A1-A3"}, {"value": "9.33404120234695E-13", "module": "A4"}, {"value": "1.99304439485045E-13", "module": "A5"}, {"value": "0", "module": "B1"}, {"value": "-1.05127912039777E-11", "module": "B2"}, {"value": "0", "module": "B6"}, {"value": "0", "module": "B7"}, {"value": "2.02039932608643E-12", "module": "C1"}, {"value": "1.81885870828448E-13", "module": "C2"}, {"value": "4.45114968016351E-11", "module": "C3", "scenario": "S1"}, {"value": "8.37507163344968E-12", "module": "C3", "scenario": "S2"}, {"value": "8.64909985920622E-11", "module": "C4"}, {"value": "-2.77142401348582E-09", "module": "D", "scenario": "S1"}, {"value": "-5.87381934982972E-09", "module": "D", "scenario": "S2"}, {"value": "0", "module": "D", "scenario": "S3"}]}, "resolvedFlowVersion": "38.00.000", "flowProperties": [], "typeOfFlow": "Other flow", "classification": {"classHierarchy": "Quantities / Environmental quantities / EPD EN 15804 / LCI indicators", "name": "GaBiCategories"}}, {"dataSetInternalID": 12, "referenceToFlowDataSet": {"shortDescription": [{"value": "Entsorgter nicht gefährlicher Abfall (NHWD)", "lang": "de"}, {"value": "Non hazardous waste disposed (NHWD)", "lang": "en"}], "type": "flow data set", "refObjectId": "b29ef66b-e286-4afa-949f-62f1a7b4d7fa", "uri": "../flows/b29ef66b-e286-4afa-949f-62f1a7b4d7fa.xml"}, "exchange direction": "OUTPUT", "other": {"anies": [{"name": "referenceToUnitGroupDataSet", "value": {"shortDescription": [{"value": "kg", "lang": "de"}], "type": "unit group data set", "refObjectId": "ad38d542-3fe9-439d-9b95-2f5f7752acaf", "uri": "../unitgroups/ad38d542-3fe9-439d-9b95-2f5f7752acaf.xml"}}, {"value": "0.0220752510604012", "module": "A1-A3"}, {"value": "8.28753238767623E-05", "module": "A4"}, {"value": "0.00119044382691754", "module": "A5"}, {"value": "0", "module": "B1"}, {"value": "0.0333624200812222", "module": "B2"}, {"value": "0", "module": "B6"}, {"value": "0", "module": "B7"}, {"value": "7.89589105145176E-05", "module": "C1"}, {"value": "8.95467876323702E-06", "module": "C2"}, {"value": "0.00142049769700847", "module": "C3", "scenario": "S1"}, {"value": "0.0124131085992543", "module": "C3", "scenario": "S2"}, {"value": "0.996041366164487", "module": "C4"}, {"value": "-0.00793583681225392", "module": "D", "scenario": "S1"}, {"value": "-0.0122134231431402", "module": "D", "scenario": "S2"}, {"value": "0", "module": "D", "scenario": "S3"}]}, "resolvedFlowVersion": "38.00.000", "flowProperties": [], "typeOfFlow": "Other flow", "classification": {"classHierarchy": "Quantities / Environmental quantities / EPD EN 15804 / LCI indicators", "name": "GaBiCategories"}}, {"dataSetInternalID": 13, "referenceToFlowDataSet": {"shortDescription": [{"value": "Entsorgter radioaktiver Abfall (RWD)", "lang": "de"}, {"value": "Radioactive waste disposed (RWD)", "lang": "en"}], "type": "flow data set", "refObjectId": "3449546e-52ad-4b39-b809-9fb77cea8ff6", "uri": "../flows/3449546e-52ad-4b39-b809-9fb77cea8ff6.xml"}, "exchange direction": "OUTPUT", "other": {"anies": [{"name": "referenceToUnitGroupDataSet", "value": {"shortDescription": [{"value": "kg", "lang": "de"}], "type": "unit group data set", "refObjectId": "ad38d542-3fe9-439d-9b95-2f5f7752acaf", "uri": "../unitgroups/ad38d542-3fe9-439d-9b95-2f5f7752acaf.xml"}}, {"value": "0.000459918053462978", "module": "A1-A3"}, {"value": "7.28886862696338E-07", "module": "A4"}, {"value": "8.05281198354054E-07", "module": "A5"}, {"value": "0", "module": "B1"}, {"value": "1.28438632902871E-05", "module": "B2"}, {"value": "0", "module": "B6"}, {"value": "0", "module": "B7"}, {"value": "7.12476026959399E-07", "module": "C1"}, {"value": "1.09933366137618E-07", "module": "C2"}, {"value": "0.000110455851215822", "module": "C3", "scenario": "S1"}, {"value": "2.24092190350671E-05", "module": "C3", "scenario": "S2"}, {"value": "1.21603158513234E-05", "module": "C4"}, {"value": "-0.000285681098798654", "module": "D", "scenario": "S1"}, {"value": "-0.00187137776606703", "module": "D", "scenario": "S2"}, {"value": "0", "module": "D", "scenario": "S3"}]}, "resolvedFlowVersion": "38.00.000", "flowProperties": [], "typeOfFlow": "Other flow", "classification": {"classHierarchy": "Quantities / Environmental quantities / EPD EN 15804 / LCI indicators", "name": "GaBiCategories"}}, {"dataSetInternalID": 14, "referenceToFlowDataSet": {"shortDescription": [{"value": "Komponenten für die Wiederverwendung (CRU)", "lang": "de"}, {"value": "Components for re-use (CRU)", "lang": "en"}], "type": "flow data set", "refObjectId": "a2b32f97-3fc7-4af2-b209-525bc6426f33", "uri": "../flows/a2b32f97-3fc7-4af2-b209-525bc6426f33.xml"}, "exchange direction": "OUTPUT", "other": {"anies": [{"name": "referenceToUnitGroupDataSet", "value": {"shortDescription": [{"value": "kg", "lang": "de"}], "type": "unit group data set", "refObjectId": "ad38d542-3fe9-439d-9b95-2f5f7752acaf", "uri": "../unitgroups/ad38d542-3fe9-439d-9b95-2f5f7752acaf.xml"}}, {"value": "0", "module": "A1-A3"}, {"value": "0", "module": "A4"}, {"value": "0", "module": "A5"}, {"value": "0", "module": "B1"}, {"value": "0", "module": "B2"}, {"value": "0", "module": "B6"}, {"value": "0", "module": "B7"}, {"value": "0", "module": "C1"}, {"value": "0", "module": "C2"}, {"value": "0", "module": "C3", "scenario": "S1"}, {"value": "0", "module": "C3", "scenario": "S2"}, {"value": "0", "module": "C4"}, {"value": "0", "module": "D", "scenario": "S1"}, {"value": "0", "module": "D", "scenario": "S2"}, {"value": "0", "module": "D", "scenario": "S3"}]}, "resolvedFlowVersion": "38.00.000", "flowProperties": [], "typeOfFlow": "Other flow", "classification": {"classHierarchy": "Quantities / Environmental quantities / EPD EN 15804 / LCI indicators", "name": "GaBiCategories"}}, {"dataSetInternalID": 15, "referenceToFlowDataSet": {"shortDescription": [{"value": "Stoffe zum Recycling (MFR)", "lang": "de"}, {"value": "Materials for recycling (MFR)", "lang": "en"}], "type": "flow data set", "refObjectId": "d7fe48a5-4103-49c8-9aae-b0b5dfdbd6ae", "uri": "../flows/d7fe48a5-4103-49c8-9aae-b0b5dfdbd6ae.xml"}, "exchange direction": "OUTPUT", "other": {"anies": [{"name": "referenceToUnitGroupDataSet", "value": {"shortDescription": [{"value": "kg", "lang": "de"}], "type": "unit group data set", "refObjectId": "ad38d542-3fe9-439d-9b95-2f5f7752acaf", "uri": "../unitgroups/ad38d542-3fe9-439d-9b95-2f5f7752acaf.xml"}}, {"value": "0.036", "module": "A1-A3"}, {"value": "0", "module": "A4"}, {"value": "0", "module": "A5"}, {"value": "0", "module": "B1"}, {"value": "0", "module": "B2"}, {"value": "0", "module": "B6"}, {"value": "0", "module": "B7"}, {"value": "0", "module": "C1"}, {"value": "0", "module": "C2"}, {"value": "0.95", "module": "C3", "scenario": "S1"}, {"value": "0", "module": "C3", "scenario": "S2"}, {"value": "0", "module": "C4"}, {"value": "0", "module": "D", "scenario": "S1"}, {"value": "0", "module": "D", "scenario": "S2"}, {"value": "0", "module": "D", "scenario": "S3"}]}, "resolvedFlowVersion": "38.00.000", "flowProperties": [], "typeOfFlow": "Other flow", "classification": {"classHierarchy": "Quantities / Environmental quantities / EPD EN 15804 / LCI indicators", "name": "GaBiCategories"}}, {"dataSetInternalID": 16, "referenceToFlowDataSet": {"shortDescription": [{"value": "Stoffe für die Energierückgewinnung (MER)", "lang": "de"}, {"value": "Materials for energy recovery (MER)", "lang": "en"}], "type": "flow data set", "refObjectId": "59a9181c-3aaf-46ee-8b13-2b3723b6e447", "uri": "../flows/59a9181c-3aaf-46ee-8b13-2b3723b6e447.xml"}, "exchange direction": "OUTPUT", "other": {"anies": [{"name": "referenceToUnitGroupDataSet", "value": {"shortDescription": [{"value": "kg", "lang": "de"}], "type": "unit group data set", "refObjectId": "ad38d542-3fe9-439d-9b95-2f5f7752acaf", "uri": "../unitgroups/ad38d542-3fe9-439d-9b95-2f5f7752acaf.xml"}}, {"value": "0", "module": "A1-A3"}, {"value": "0", "module": "A4"}, {"value": "0", "module": "A5"}, {"value": "0", "module": "B1"}, {"value": "0", "module": "B2"}, {"value": "0", "module": "B6"}, {"value": "0", "module": "B7"}, {"value": "0", "module": "C1"}, {"value": "0", "module": "C2"}, {"value": "0", "module": "C3", "scenario": "S1"}, {"value": "0", "module": "C3", "scenario": "S2"}, {"value": "0", "module": "C4"}, {"value": "0", "module": "D", "scenario": "S1"}, {"value": "0", "module": "D", "scenario": "S2"}, {"value": "0", "module": "D", "scenario": "S3"}]}, "resolvedFlowVersion": "38.00.000", "flowProperties": [], "typeOfFlow": "Other flow", "classification": {"classHierarchy": "Quantities / Environmental quantities / EPD EN 15804 / LCI indicators", "name": "GaBiCategories"}}, {"dataSetInternalID": 17, "referenceToFlowDataSet": {"shortDescription": [{"value": "Exportierte elektrische Energie (EEE)", "lang": "de"}, {"value": "Exported electrical energy (EEE)", "lang": "en"}], "type": "flow data set", "refObjectId": "4da0c987-2b76-40d6-9e9e-82a017aaaf29", "uri": "../flows/4da0c987-2b76-40d6-9e9e-82a017aaaf29.xml"}, "exchange direction": "OUTPUT", "other": {"anies": [{"name": "referenceToUnitGroupDataSet", "value": {"shortDescription": [{"value": "MJ", "lang": "de"}], "type": "unit group data set", "refObjectId": "93a60a57-a3c8-11da-a746-0800200c9a66", "uri": "../unitgroups/93a60a57-a3c8-11da-a746-0800200c9a66.xml"}}, {"value": "0.0153", "module": "A1-A3"}, {"value": "0", "module": "A4"}, {"value": "0.0955", "module": "A5"}, {"value": "0", "module": "B1"}, {"value": "0", "module": "B2"}, {"value": "0", "module": "B6"}, {"value": "0", "module": "B7"}, {"value": "0", "module": "C1"}, {"value": "0", "module": "C2"}, {"value": "0.334", "module": "C3", "scenario": "S1"}, {"value": "6.68113999843291", "module": "C3", "scenario": "S2"}, {"value": "0", "module": "C4"}, {"value": "0", "module": "D", "scenario": "S1"}, {"value": "0", "module": "D", "scenario": "S2"}, {"value": "0", "module": "D", "scenario": "S3"}]}, "resolvedFlowVersion": "38.00.000", "flowProperties": [], "typeOfFlow": "Other flow", "classification": {"classHierarchy": "Quantities / Environmental quantities / EPD EN 15804 / LCI indicators", "name": "GaBiCategories"}}, {"dataSetInternalID": 18, "referenceToFlowDataSet": {"shortDescription": [{"value": "Exportierte thermische Energie (EET)", "lang": "de"}, {"value": "Exported thermal energy (EET)", "lang": "en"}], "type": "flow data set", "refObjectId": "98daf38a-7a79-46d3-9a37-2b7bd0955810", "uri": "../flows/98daf38a-7a79-46d3-9a37-2b7bd0955810.xml"}, "exchange direction": "OUTPUT", "other": {"anies": [{"name": "referenceToUnitGroupDataSet", "value": {"shortDescription": [{"value": "MJ", "lang": "de"}], "type": "unit group data set", "refObjectId": "93a60a57-a3c8-11da-a746-0800200c9a66", "uri": "../unitgroups/93a60a57-a3c8-11da-a746-0800200c9a66.xml"}}, {"value": "0.0288", "module": "A1-A3"}, {"value": "0", "module": "A4"}, {"value": "0.225", "module": "A5"}, {"value": "0", "module": "B1"}, {"value": "0", "module": "B2"}, {"value": "0", "module": "B6"}, {"value": "0", "module": "B7"}, {"value": "0", "module": "C1"}, {"value": "0", "module": "C2"}, {"value": "0.594", "module": "C3", "scenario": "S1"}, {"value": "11.8799848225502", "module": "C3", "scenario": "S2"}, {"value": "0", "module": "C4"}, {"value": "0", "module": "D", "scenario": "S1"}, {"value": "0", "module": "D", "scenario": "S2"}, {"value": "0", "module": "D", "scenario": "S3"}]}, "resolvedFlowVersion": "38.00.000", "flowProperties": [], "typeOfFlow": "Other flow", "classification": {"classHierarchy": "Quantities / Environmental quantities / EPD EN 15804 / LCI indicators", "name": "GaBiCategories"}}]}, "LCIAResults": {"LCIAResult": [{"referenceToLCIAMethodDataSet": {"shortDescription": [{"value": "Globales Erwärmungspotenzial total (GWP-total)", "lang": "de"}, {"value": "Global Warming Potential total (GWP-total)", "lang": "en"}], "type": "LCIA method data set", "refObjectId": "6a37f984-a4b3-458a-a20a-64418c145fa2", "uri": "../lciamethods/6a37f984-a4b3-458a-a20a-64418c145fa2.xml"}, "other": {"anies": [{"name": "referenceToUnitGroupDataSet", "value": {"shortDescription": [{"value": "kg CO_(2)-Äq.", "lang": "de"}], "type": "unit group data set", "refObjectId": "1ebf3012-d0db-4de2-aefd-ef30cedb0be1", "uri": "../unitgroups/1ebf3012-d0db-4de2-aefd-ef30cedb0be1.xml"}}, {"value": "1.93270721912758", "module": "A1-A3"}, {"value": "0.0405357817040383", "module": "A4"}, {"value": "0.0823015931785808", "module": "A5"}, {"value": "0", "module": "B1"}, {"value": "0.178720090922366", "module": "B2"}, {"value": "0", "module": "B6"}, {"value": "0", "module": "B7"}, {"value": "0.0406009619720366", "module": "C1"}, {"value": "0.00429396629798976", "module": "C2"}, {"value": "0.246339222704853", "module": "C3", "scenario": "S1"}, {"value": "3.13004958430526", "module": "C3", "scenario": "S2"}, {"value": "0.0677526434063481", "module": "C4"}, {"value": "-0.873342366986997", "module": "D", "scenario": "S1"}, {"value": "-1.49621638155984", "module": "D", "scenario": "S2"}, {"value": "0", "module": "D", "scenario": "S3"}]}}, {"referenceToLCIAMethodDataSet": {"shortDescription": [{"value": "Globales Erwärmungspotenzial fossil (GWP-fossil)", "lang": "de"}, {"value": "Global Warming Potential fossil fuels (GWP-fossil)", "lang": "en"}], "type": "LCIA method data set", "refObjectId": "5f635281-343e-44fb-83df-1971b155e6b6", "uri": "../lciamethods/5f635281-343e-44fb-83df-1971b155e6b6.xml"}, "other": {"anies": [{"name": "referenceToUnitGroupDataSet", "value": {"shortDescription": [{"value": "kg CO_(2)-Äq.", "lang": "de"}], "type": "unit group data set", "refObjectId": "1ebf3012-d0db-4de2-aefd-ef30cedb0be1", "uri": "../unitgroups/1ebf3012-d0db-4de2-aefd-ef30cedb0be1.xml"}}, {"value": "1.99516702513472", "module": "A1-A3"}, {"value": "0.0404747230204318", "module": "A4"}, {"value": "0.00259862394527521", "module": "A5"}, {"value": "0", "module": "B1"}, {"value": "0.160730877198558", "module": "B2"}, {"value": "0", "module": "B6"}, {"value": "0", "module": "B7"}, {"value": "0.0407868158099233", "module": "C1"}, {"value": "0.00431750534325615", "module": "C2"}, {"value": "0.246285605574908", "module": "C3", "scenario": "S1"}, {"value": "3.12996281524702", "module": "C3", "scenario": "S2"}, {"value": "0.0685415812020125", "module": "C4"}, {"value": "-0.86830059135236", "module": "D", "scenario": "S1"}, {"value": "-1.48916551824518", "module": "D", "scenario": "S2"}, {"value": "0", "module": "D", "scenario": "S3"}]}}, {"referenceToLCIAMethodDataSet": {"shortDescription": [{"value": "Globales Erwärmungspotenzial biogen (GWP-biogenic)", "lang": "de"}, {"value": "Global Warming Potential biogenic (GWP-biogenic)", "lang": "en"}], "type": "LCIA method data set", "refObjectId": "2356e1ab-0185-4db5-86e5-16de51c7485c", "uri": "../lciamethods/2356e1ab-0185-4db5-86e5-16de51c7485c.xml"}, "other": {"anies": [{"name": "referenceToUnitGroupDataSet", "value": {"shortDescription": [{"value": "kg CO_(2)-Äq.", "lang": "de"}], "type": "unit group data set", "refObjectId": "1ebf3012-d0db-4de2-aefd-ef30cedb0be1", "uri": "../unitgroups/1ebf3012-d0db-4de2-aefd-ef30cedb0be1.xml"}}, {"value": "-0.0631691113331346", "module": "A1-A3"}, {"value": "-0.000182129786567727", "module": "A4"}, {"value": "0.0796802836697581", "module": "A5"}, {"value": "0", "module": "B1"}, {"value": "0.0179799186364914", "module": "B2"}, {"value": "0", "module": "B6"}, {"value": "0", "module": "B7"}, {"value": "-0.000557702595392008", "module": "C1"}, {"value": "-6.33255148769523E-05", "module": "C2"}, {"value": "4.52969089394335E-05", "module": "C3", "scenario": "S1"}, {"value": "8.36779452348278E-05", "module": "C3", "scenario": "S2"}, {"value": "-0.000845544078701924", "module": "C4"}, {"value": "-0.004871676107897", "module": "D", "scenario": "S1"}, {"value": "-0.00601529065024964", "module": "D", "scenario": "S2"}, {"value": "0", "module": "D", "scenario": "S3"}]}}, {"referenceToLCIAMethodDataSet": {"shortDescription": [{"value": "Globales Erwärmungspotenzial luluc (GWP-luluc)", "lang": "de"}, {"value": "Global Warming Potential luluc (GWP-luluc)", "lang": "en"}], "type": "LCIA method data set", "refObjectId": "4331bbdb-978a-490d-8707-eeb047f01a55", "uri": "../lciamethods/4331bbdb-978a-490d-8707-eeb047f01a55.xml"}, "other": {"anies": [{"name": "referenceToUnitGroupDataSet", "value": {"shortDescription": [{"value": "kg CO_(2)-Äq.", "lang": "de"}], "type": "unit group data set", "refObjectId": "1ebf3012-d0db-4de2-aefd-ef30cedb0be1", "uri": "../unitgroups/1ebf3012-d0db-4de2-aefd-ef30cedb0be1.xml"}}, {"value": "0.000709305325992962", "module": "A1-A3"}, {"value": "0.000243188470174199", "module": "A4"}, {"value": "2.26855635475162E-05", "module": "A5"}, {"value": "0", "module": "B1"}, {"value": "9.29508731650895E-06", "module": "B2"}, {"value": "0", "module": "B6"}, {"value": "0", "module": "B7"}, {"value": "0.000371848757505334", "module": "C1"}, {"value": "3.97864696105658E-05", "module": "C2"}, {"value": "8.32022100562685E-06", "module": "C3", "scenario": "S1"}, {"value": "3.09111300634013E-06", "module": "C3", "scenario": "S2"}, {"value": "5.66062830374693E-05", "module": "C4"}, {"value": "-0.00017009952673983", "module": "D", "scenario": "S1"}, {"value": "-0.00103557266441128", "module": "D", "scenario": "S2"}, {"value": "0", "module": "D", "scenario": "S3"}]}}, {"referenceToLCIAMethodDataSet": {"shortDescription": [{"value": "Abbau Potential der stratosphärischen Ozonschicht (ODP)", "lang": "de"}, {"value": "Depletion potential of the stratospheric ozone layer (ODP)", "lang": "en"}], "type": "LCIA method data set", "refObjectId": "b5c629d6-def3-11e6-bf01-fe55135034f3", "uri": "../lciamethods/b5c629d6-def3-11e6-bf01-fe55135034f3.xml"}, "other": {"anies": [{"name": "referenceToUnitGroupDataSet", "value": {"shortDescription": [{"value": "kg CFC11-Äq.", "lang": "de"}], "type": "unit group data set", "refObjectId": "d9e957c9-7309-4474-bf3a-7777df6c4e5b", "uri": "../unitgroups/d9e957c9-7309-4474-bf3a-7777df6c4e5b.xml"}}, {"value": "2.24637376457664E-11", "module": "A1-A3"}, {"value": "1.00303487773828E-14", "module": "A4"}, {"value": "1.55260644102513E-14", "module": "A5"}, {"value": "0", "module": "B1"}, {"value": "2.44284629962471E-13", "module": "B2"}, {"value": "0", "module": "B6"}, {"value": "0", "module": "B7"}, {"value": "3.54069331000658E-15", "module": "C1"}, {"value": "5.58973268073841E-16", "module": "C2"}, {"value": "1.23904731045349E-14", "module": "C3", "scenario": "S1"}, {"value": "1.48167753727999E-13", "module": "C3", "scenario": "S2"}, {"value": "1.15568745477024E-13", "module": "C4"}, {"value": "-2.83726039012511E-12", "module": "D", "scenario": "S1"}, {"value": "-1.70412381884345E-14", "module": "D", "scenario": "S2"}, {"value": "0", "module": "D", "scenario": "S3"}]}}, {"referenceToLCIAMethodDataSet": {"shortDescription": [{"value": "Versauerungspotenzial von Boden und Wasser (AP)", "lang": "de"}, {"value": "Acidification potential of land and water (AP)", "lang": "en"}], "type": "LCIA method data set", "refObjectId": "b5c611c6-def3-11e6-bf01-fe55135034f3", "uri": "../lciamethods/b5c611c6-def3-11e6-bf01-fe55135034f3.xml"}, "other": {"anies": [{"name": "referenceToUnitGroupDataSet", "value": {"shortDescription": [{"value": "mol H^(+)-Äq.", "lang": "de"}], "type": "unit group data set", "refObjectId": "42e089ac-92bf-4bf2-8ca1-5fc40d18f2ed", "uri": "../unitgroups/42e089ac-92bf-4bf2-8ca1-5fc40d18f2ed.xml"}}, {"value": "0.00342051649641459", "module": "A1-A3"}, {"value": "5.46117102335912E-05", "module": "A4"}, {"value": "1.96377106990466E-05", "module": "A5"}, {"value": "0", "module": "B1"}, {"value": "0.000193331147599058", "module": "B2"}, {"value": "0", "module": "B6"}, {"value": "0", "module": "B7"}, {"value": "0.000205766404495031", "module": "C1"}, {"value": "6.40401688536925E-06", "module": "C2"}, {"value": "0.000168244869990664", "module": "C3", "scenario": "S1"}, {"value": "0.000308746578643678", "module": "C3", "scenario": "S2"}, {"value": "0.000206298507684426", "module": "C4"}, {"value": "-0.00128074020103051", "module": "D", "scenario": "S1"}, {"value": "-0.00195399649247697", "module": "D", "scenario": "S2"}, {"value": "0", "module": "D", "scenario": "S3"}]}}, {"referenceToLCIAMethodDataSet": {"shortDescription": [{"value": "Eutrophierungspotenzial Süßwasser (EP-freshwater)", "lang": "de"}, {"value": "Eutrophication potential aquatic freshwater (EP-freshwater)", "lang": "en"}], "type": "LCIA method data set", "refObjectId": "b53ec18f-7377-4ad3-86eb-cc3f4f276b2b", "uri": "../lciamethods/b53ec18f-7377-4ad3-86eb-cc3f4f276b2b.xml"}, "other": {"anies": [{"name": "referenceToUnitGroupDataSet", "value": {"shortDescription": [{"value": "kg P-Äq.", "lang": "de"}], "type": "unit group data set", "refObjectId": "0429039d-a61d-4590-ba67-aa4a20a810a1", "uri": "../unitgroups/0429039d-a61d-4590-ba67-aa4a20a810a1.xml"}}, {"value": "6.3915795324422E-06", "module": "A1-A3"}, {"value": "9.58283181852846E-08", "module": "A4"}, {"value": "1.262640302392E-08", "module": "A5"}, {"value": "0", "module": "B1"}, {"value": "2.09640538429754E-05", "module": "B2"}, {"value": "0", "module": "B6"}, {"value": "0", "module": "B7"}, {"value": "1.46402053417942E-07", "module": "C1"}, {"value": "1.5706377347662E-08", "module": "C2"}, {"value": "4.42031070301795E-08", "module": "C3", "scenario": "S1"}, {"value": "3.51417035438723E-08", "module": "C3", "scenario": "S2"}, {"value": "1.32371254234767E-05", "module": "C4"}, {"value": "-1.28741179305129E-06", "module": "D", "scenario": "S1"}, {"value": "-1.95715968429049E-06", "module": "D", "scenario": "S2"}, {"value": "0", "module": "D", "scenario": "S3"}]}}, {"referenceToLCIAMethodDataSet": {"shortDescription": [{"value": "Eutrophierungspotenzial Salzwasser (EP-marine)", "lang": "de"}, {"value": "Eutrophication potential aquatic marine (EP-marine)", "lang": "en"}], "type": "LCIA method data set", "refObjectId": "b5c619fa-def3-11e6-bf01-fe55135034f3", "uri": "../lciamethods/b5c619fa-def3-11e6-bf01-fe55135034f3.xml"}, "other": {"anies": [{"name": "referenceToUnitGroupDataSet", "value": {"shortDescription": [{"value": "kg N-Äq.", "lang": "de"}], "type": "unit group data set", "refObjectId": "d05bb823-ecdf-4686-8c40-bf1d9257859f", "uri": "../unitgroups/d05bb823-ecdf-4686-8c40-bf1d9257859f.xml"}}, {"value": "0.00091417877499192", "module": "A1-A3"}, {"value": "2.04760319016793E-05", "module": "A4"}, {"value": "5.14392214949215E-06", "module": "A5"}, {"value": "0", "module": "B1"}, {"value": "0.00014967798850786", "module": "B2"}, {"value": "0", "module": "B6"}, {"value": "0", "module": "B7"}, {"value": "9.68483716011057E-05", "module": "C1"}, {"value": "2.33555840643605E-06", "module": "C2"}, {"value": "4.34858633217938E-05", "module": "C3", "scenario": "S1"}, {"value": "6.46834424541432E-05", "module": "C3", "scenario": "S2"}, {"value": "4.72600360811732E-05", "module": "C4"}, {"value": "-0.000367357189602324", "module": "D", "scenario": "S1"}, {"value": "-0.000557738521658963", "module": "D", "scenario": "S2"}, {"value": "0", "module": "D", "scenario": "S3"}]}}, {"referenceToLCIAMethodDataSet": {"shortDescription": [{"value": "Eutrophierungspotenzial Land (EP-terrestrial)", "lang": "de"}, {"value": "Eutrophication potential terrestrial (EP-terrestrial)", "lang": "en"}], "type": "LCIA method data set", "refObjectId": "b5c614d2-def3-11e6-bf01-fe55135034f3", "uri": "../lciamethods/b5c614d2-def3-11e6-bf01-fe55135034f3.xml"}, "other": {"anies": [{"name": "referenceToUnitGroupDataSet", "value": {"shortDescription": [{"value": "mol N-Äq.", "lang": "de"}], "type": "unit group data set", "refObjectId": "71b4d617-0ec9-4d3f-b65e-e438940c2401", "uri": "../unitgroups/71b4d617-0ec9-4d3f-b65e-e438940c2401.xml"}}, {"value": "0.00965611228084039", "module": "A1-A3"}, {"value": "0.000242143287024555", "module": "A4"}, {"value": "8.26603089028077E-05", "module": "A5"}, {"value": "0", "module": "B1"}, {"value": "0.00074132350860397", "module": "B2"}, {"value": "0", "module": "B6"}, {"value": "0", "module": "B7"}, {"value": "0.00107333008093773", "module": "C1"}, {"value": "2.76085953671117E-05", "module": "C2"}, {"value": "0.000508894334473568", "module": "C3", "scenario": "S1"}, {"value": "0.00145491473913303", "module": "C3", "scenario": "S2"}, {"value": "0.000518926563367949", "module": "C4"}, {"value": "-0.0038811517375569", "module": "D", "scenario": "S1"}, {"value": "-0.00597646234835113", "module": "D", "scenario": "S2"}, {"value": "0", "module": "D", "scenario": "S3"}]}}, {"referenceToLCIAMethodDataSet": {"shortDescription": [{"value": "Bildungspotential für troposphärisches Ozon (POCP)", "lang": "de"}, {"value": "Formation potential of tropospheric ozone photochemical oxidants (POCP)", "lang": "en"}], "type": "LCIA method data set", "refObjectId": "b5c610fe-def3-11e6-bf01-fe55135034f3", "uri": "../lciamethods/b5c610fe-def3-11e6-bf01-fe55135034f3.xml"}, "other": {"anies": [{"name": "referenceToUnitGroupDataSet", "value": {"shortDescription": [{"value": "kg NMVOC-Äq.", "lang": "de"}], "type": "unit group data set", "refObjectId": "d27c25f8-fbc1-44c6-b47b-4adbae4199c6", "uri": "../unitgroups/d27c25f8-fbc1-44c6-b47b-4adbae4199c6.xml"}}, {"value": "0.00336643237100222", "module": "A1-A3"}, {"value": "4.84773741919421E-05", "module": "A4"}, {"value": "1.37034659728995E-05", "module": "A5"}, {"value": "0", "module": "B1"}, {"value": "0.000200019351358789", "module": "B2"}, {"value": "0", "module": "B6"}, {"value": "0", "module": "B7"}, {"value": "0.000271730978145597", "module": "C1"}, {"value": "5.62267498794181E-06", "module": "C2"}, {"value": "0.000122280485745574", "module": "C3", "scenario": "S1"}, {"value": "0.000192448304791373", "module": "C3", "scenario": "S2"}, {"value": "0.000150104779094988", "module": "C4"}, {"value": "-0.00143655899059238", "module": "D", "scenario": "S1"}, {"value": "-0.00156621250279568", "module": "D", "scenario": "S2"}, {"value": "0", "module": "D", "scenario": "S3"}]}}, {"referenceToLCIAMethodDataSet": {"shortDescription": [{"value": "Potenzial für den abiotischen Abbau nicht fossiler Ressourcen (ADPE)", "lang": "de"}, {"value": "Abiotic depletion potential for non fossil resources (ADPE)", "lang": "en"}], "type": "LCIA method data set", "refObjectId": "b2ad6494-c78d-11e6-9d9d-cec0c932ce01", "uri": "../lciamethods/b2ad6494-c78d-11e6-9d9d-cec0c932ce01.xml"}, "other": {"anies": [{"name": "referenceToUnitGroupDataSet", "value": {"shortDescription": [{"value": "kg Sb-Äq.", "lang": "de"}], "type": "unit group data set", "refObjectId": "54ccd2d9-a32a-4fc2-923d-f2c8c93e89d4", "uri": "../unitgroups/54ccd2d9-a32a-4fc2-923d-f2c8c93e89d4.xml"}}, {"value": "6.60869515989809E-07", "module": "A1-A3"}, {"value": "2.94235489099806E-09", "module": "A4"}, {"value": "3.79818131494682E-10", "module": "A5"}, {"value": "0", "module": "B1"}, {"value": "2.88175350638748E-09", "module": "B2"}, {"value": "0", "module": "B6"}, {"value": "0", "module": "B7"}, {"value": "2.60844129771909E-09", "module": "C1"}, {"value": "2.8482244005484E-10", "module": "C2"}, {"value": "9.81369354927441E-10", "module": "C3", "scenario": "S1"}, {"value": "1.37817489550319E-09", "module": "C3", "scenario": "S2"}, {"value": "1.81861227028962E-09", "module": "C4"}, {"value": "-5.27336962313877E-08", "module": "D", "scenario": "S1"}, {"value": "-2.49147634451351E-07", "module": "D", "scenario": "S2"}, {"value": "0", "module": "D", "scenario": "S3"}]}}, {"referenceToLCIAMethodDataSet": {"shortDescription": [{"value": "Potenzial für den abiotischen Abbau fossiler Brennstoffe (ADPF)", "lang": "de"}, {"value": "Abiotic depletion potential for fossil resources (ADPF)", "lang": "en"}], "type": "LCIA method data set", "refObjectId": "b2ad6110-c78d-11e6-9d9d-cec0c932ce01", "uri": "../lciamethods/b2ad6110-c78d-11e6-9d9d-cec0c932ce01.xml"}, "other": {"anies": [{"name": "referenceToUnitGroupDataSet", "value": {"shortDescription": [{"value": "MJ", "lang": "de"}], "type": "unit group data set", "refObjectId": "93a60a57-a3c8-11da-a746-0800200c9a66", "uri": "../unitgroups/93a60a57-a3c8-11da-a746-0800200c9a66.xml"}}, {"value": "70.8014813417506", "module": "A1-A3"}, {"value": "0.552696188380548", "module": "A4"}, {"value": "0.0725200115023128", "module": "A5"}, {"value": "0", "module": "B1"}, {"value": "2.07083317333624", "module": "B2"}, {"value": "0", "module": "B6"}, {"value": "0", "module": "B7"}, {"value": "0.545961513443688", "module": "C1"}, {"value": "0.0585212402376255", "module": "C2"}, {"value": "1.36856531491483", "module": "C3", "scenario": "S1"}, {"value": "0.372093370014288", "module": "C3", "scenario": "S2"}, {"value": "1.02655419337746", "module": "C4"}, {"value": "-33.5686524957664", "module": "D", "scenario": "S1"}, {"value": "-26.1325532566803", "module": "D", "scenario": "S2"}, {"value": "0", "module": "D", "scenario": "S3"}]}}, {"referenceToLCIAMethodDataSet": {"shortDescription": [{"value": "Wassernutzung (WDP)", "lang": "de"}, {"value": "Water use (WDP)", "lang": "en"}], "type": "LCIA method data set", "refObjectId": "b2ad66ce-c78d-11e6-9d9d-cec0c932ce01", "uri": "../lciamethods/b2ad66ce-c78d-11e6-9d9d-cec0c932ce01.xml"}, "other": {"anies": [{"name": "referenceToUnitGroupDataSet", "value": {"shortDescription": [{"value": "m^(3) Welt-Äq. entzogen", "lang": "de"}], "type": "unit group data set", "refObjectId": "6ae2df01-888e-46c8-b17d-49fa3869b476", "uri": "../unitgroups/6ae2df01-888e-46c8-b17d-49fa3869b476.xml"}}, {"value": "0.11102464292105", "module": "A1-A3"}, {"value": "0.000213440125381341", "module": "A4"}, {"value": "0.00890192044591946", "module": "A5"}, {"value": "0", "module": "B1"}, {"value": "0.00285644336529592", "module": "B2"}, {"value": "0", "module": "B6"}, {"value": "0", "module": "B7"}, {"value": "0.000463083106655885", "module": "C1"}, {"value": "5.19109396885471E-05", "module": "C2"}, {"value": "0.0865501717524717", "module": "C3", "scenario": "S1"}, {"value": "0.288719911945024", "module": "C3", "scenario": "S2"}, {"value": "-0.000970803233614453", "module": "C4"}, {"value": "-0.0541510751388152", "module": "D", "scenario": "S1"}, {"value": "-0.112883403977222", "module": "D", "scenario": "S2"}, {"value": "0", "module": "D", "scenario": "S3"}]}}, {"referenceToLCIAMethodDataSet": {"shortDescription": [{"value": "Auftreten von Krankheiten aufgrund von Feinstaubemissionen (PM)", "lang": "de"}, {"value": "Incidence of disease due to PM emissions (PM)", "lang": "en"}], "type": "LCIA method data set", "refObjectId": "b5c602c6-def3-11e6-bf01-fe55135034f3", "uri": "../lciamethods/b5c602c6-def3-11e6-bf01-fe55135034f3.xml"}, "other": {"anies": [{"name": "referenceToUnitGroupDataSet", "value": {"shortDescription": [{"value": "Krankheitsfälle", "lang": "de"}], "type": "unit group data set", "refObjectId": "3883559b-648f-4afc-8ba2-0bd24f3affa3", "uri": "../unitgroups/3883559b-648f-4afc-8ba2-0bd24f3affa3.xml"}}, {"value": "4.60506480282134E-08", "module": "A1-A3"}, {"value": "4.4840394121877E-10", "module": "A4"}, {"value": "1.33495007085289E-10", "module": "A5"}, {"value": "0", "module": "B1"}, {"value": "1.30270980419349E-09", "module": "B2"}, {"value": "0", "module": "B6"}, {"value": "0", "module": "B7"}, {"value": "2.32441328880595E-09", "module": "C1"}, {"value": "5.30209341210527E-11", "module": "C2"}, {"value": "1.42689447992242E-09", "module": "C3", "scenario": "S1"}, {"value": "1.80956831722374E-09", "module": "C3", "scenario": "S2"}, {"value": "1.99976659237959E-09", "module": "C4"}, {"value": "-8.89342223995383E-09", "module": "D", "scenario": "S1"}, {"value": "-1.68155013521182E-08", "module": "D", "scenario": "S2"}, {"value": "0", "module": "D", "scenario": "S3"}]}}, {"referenceToLCIAMethodDataSet": {"shortDescription": [{"value": "Wirkung durch Exposition des Menschen mit U235 (IR)", "lang": "de"}, {"value": "Human exposure efficiency relative to U235 (IR)", "lang": "en"}], "type": "LCIA method data set", "refObjectId": "b5c632be-def3-11e6-bf01-fe55135034f3", "uri": "../lciamethods/b5c632be-def3-11e6-bf01-fe55135034f3.xml"}, "other": {"anies": [{"name": "referenceToUnitGroupDataSet", "value": {"shortDescription": [{"value": "kBq U235-Äq.", "lang": "de"}], "type": "unit group data set", "refObjectId": "456b05bf-1415-44a9-9993-02452f554c09", "uri": "../unitgroups/456b05bf-1415-44a9-9993-02452f554c09.xml"}}, {"value": "0.0585473656625675", "module": "A1-A3"}, {"value": "7.80783392826314E-05", "module": "A4"}, {"value": "8.5198195254226E-05", "module": "A5"}, {"value": "0", "module": "B1"}, {"value": "0.00133357600348376", "module": "B2"}, {"value": "0", "module": "B6"}, {"value": "0", "module": "B7"}, {"value": "0.000102905750050187", "module": "C1"}, {"value": "1.63939222248844E-05", "module": "C2"}, {"value": "0.0102495801606372", "module": "C3", "scenario": "S1"}, {"value": "0.00361961243374557", "module": "C3", "scenario": "S2"}, {"value": "0.0017981633363713", "module": "C4"}, {"value": "-0.0402459607367082", "module": "D", "scenario": "S1"}, {"value": "-0.306471924486741", "module": "D", "scenario": "S2"}, {"value": "0", "module": "D", "scenario": "S3"}]}}, {"referenceToLCIAMethodDataSet": {"shortDescription": [{"value": "Toxizitätsvergleichseinheit für Ökosysteme (ETP-fw)", "lang": "de"}, {"value": "Comparative toxic unit for ecosystems (ETP-fw)", "lang": "en"}], "type": "LCIA method data set", "refObjectId": "ee1082d1-b0f7-43ca-a1f0-21e2a4a74511", "uri": "../lciamethods/ee1082d1-b0f7-43ca-a1f0-21e2a4a74511.xml"}, "other": {"anies": [{"name": "referenceToUnitGroupDataSet", "value": {"shortDescription": [{"value": "CTUe", "lang": "de"}], "type": "unit group data set", "refObjectId": "aa959ded-f1eb-4efb-9c5c-2d60be36b3e6", "uri": "../unitgroups/aa959ded-f1eb-4efb-9c5c-2d60be36b3e6.xml"}}, {"value": "37.0815134439301", "module": "A1-A3"}, {"value": "0.403489968954675", "module": "A4"}, {"value": "0.0454869195731104", "module": "A5"}, {"value": "0", "module": "B1"}, {"value": "2.3358967676818", "module": "B2"}, {"value": "0", "module": "B6"}, {"value": "0", "module": "B7"}, {"value": "0.384657528507084", "module": "C1"}, {"value": "0.0419217015189163", "module": "C2"}, {"value": "0.184776588771497", "module": "C3", "scenario": "S1"}, {"value": "0.146221438722909", "module": "C3", "scenario": "S2"}, {"value": "0.876216489158938", "module": "C4"}, {"value": "-15.7040577466583", "module": "D", "scenario": "S1"}, {"value": "-3.60027784545998", "module": "D", "scenario": "S2"}, {"value": "0", "module": "D", "scenario": "S3"}]}}, {"referenceToLCIAMethodDataSet": {"shortDescription": [{"value": "Toxizitätsvergleichseinheit für Menschen (krebserregend) (HTP-c)", "lang": "de"}, {"value": "Comparative toxic unit for humans (carcinogenic) (HTP-c)", "lang": "en"}], "type": "LCIA method data set", "refObjectId": "2299222a-bbd8-474f-9d4f-4dd1f18aea7c", "uri": "../lciamethods/2299222a-bbd8-474f-9d4f-4dd1f18aea7c.xml"}, "other": {"anies": [{"name": "referenceToUnitGroupDataSet", "value": {"shortDescription": [{"value": "CTUh", "lang": "de"}], "type": "unit group data set", "refObjectId": "d4c9523e-2d7e-49fd-8469-998f547d3a70", "uri": "../unitgroups/d4c9523e-2d7e-49fd-8469-998f547d3a70.xml"}}, {"value": "9.64848964147207E-10", "module": "A1-A3"}, {"value": "8.04402543519285E-12", "module": "A4"}, {"value": "1.52670311716187E-12", "module": "A5"}, {"value": "0", "module": "B1"}, {"value": "1.3803988928201E-10", "module": "B2"}, {"value": "0", "module": "B6"}, {"value": "0", "module": "B7"}, {"value": "7.75252303976035E-12", "module": "C1"}, {"value": "8.5052804204217E-13", "module": "C2"}, {"value": "9.22425346965712E-12", "module": "C3", "scenario": "S1"}, {"value": "2.03462703110243E-11", "module": "C3", "scenario": "S2"}, {"value": "4.49745266260504E-11", "module": "C4"}, {"value": "-3.85869377490837E-10", "module": "D", "scenario": "S1"}, {"value": "-2.48416257906868E-10", "module": "D", "scenario": "S2"}, {"value": "0", "module": "D", "scenario": "S3"}]}}, {"referenceToLCIAMethodDataSet": {"shortDescription": [{"value": "Toxizitätsvergleichseinheit für Menschen (nicht krebserregend) (HTP-nc)", "lang": "de"}, {"value": "Comparative toxic unit for humans (noncarcinogenic) (HTP-nc)", "lang": "en"}], "type": "LCIA method data set", "refObjectId": "3af763a5-b7a1-48c9-9cee-1f223481fcef", "uri": "../lciamethods/3af763a5-b7a1-48c9-9cee-1f223481fcef.xml"}, "other": {"anies": [{"name": "referenceToUnitGroupDataSet", "value": {"shortDescription": [{"value": "CTUh", "lang": "de"}], "type": "unit group data set", "refObjectId": "d4c9523e-2d7e-49fd-8469-998f547d3a70", "uri": "../unitgroups/d4c9523e-2d7e-49fd-8469-998f547d3a70.xml"}}, {"value": "2.97424192172888E-08", "module": "A1-A3"}, {"value": "3.37244979821711E-10", "module": "A4"}, {"value": "6.60166158812125E-11", "module": "A5"}, {"value": "0", "module": "B1"}, {"value": "1.11422074092318E-08", "module": "B2"}, {"value": "0", "module": "B6"}, {"value": "0", "module": "B7"}, {"value": "3.43243878113028E-10", "module": "C1"}, {"value": "3.78434222209179E-11", "module": "C2"}, {"value": "3.1779915563523E-10", "module": "C3", "scenario": "S1"}, {"value": "1.522706229261E-10", "module": "C3", "scenario": "S2"}, {"value": "3.59103568085297E-09", "module": "C4"}, {"value": "-1.38872279665931E-08", "module": "D", "scenario": "S1"}, {"value": "-7.97230972775494E-09", "module": "D", "scenario": "S2"}, {"value": "0", "module": "D", "scenario": "S3"}]}}, {"referenceToLCIAMethodDataSet": {"shortDescription": [{"value": "Bodenqualitätsindex (SQP)", "lang": "de"}, {"value": "Soil quality index (SQP)", "lang": "en"}], "type": "LCIA method data set", "refObjectId": "b2ad6890-c78d-11e6-9d9d-cec0c932ce01", "uri": "../lciamethods/b2ad6890-c78d-11e6-9d9d-cec0c932ce01.xml"}, "other": {"anies": [{"name": "referenceToUnitGroupDataSet", "value": {"shortDescription": [{"value": "SQP", "lang": "de"}], "type": "unit group data set", "refObjectId": "f130951c-e67f-4f7f-8dd4-665de3974e18", "uri": "../unitgroups/f130951c-e67f-4f7f-8dd4-665de3974e18.xml"}}, {"value": "25.2905717244354", "module": "A1-A3"}, {"value": "0.196744652040834", "module": "A4"}, {"value": "0.0256723359500406", "module": "A5"}, {"value": "0", "module": "B1"}, {"value": "0.0911549860939219", "module": "B2"}, {"value": "0", "module": "B6"}, {"value": "0", "module": "B7"}, {"value": "0.227807808844405", "module": "C1"}, {"value": "0.0244525302986281", "module": "C2"}, {"value": "0.1175814476397", "module": "C3", "scenario": "S1"}, {"value": "0.117295629849174", "module": "C3", "scenario": "S2"}, {"value": "0.0889123355231071", "module": "C4"}, {"value": "-1.27137858109552", "module": "D", "scenario": "S1"}, {"value": "-4.0122691541101", "module": "D", "scenario": "S2"}, {"value": "0", "module": "D", "scenario": "S3"}]}}]}, "otherAttributes": {"{http://www.indata.network/EPD/2019}epd-version": "1.2"}, "version": "1.1", "locations": "../ILCDLocations.xml"}